Environmental product declaration
in accordance with ISO 14025 and EN 15804+A2
Sto-InnoDrain
Owner of the declaration: Program operator:
Sto SE & Co. KGaA The Norwegian EPD Foundation
Product: Declaration number:
Sto-InnoDrain
NEPD-8428-8099-EN
Declared unit:
1 m2 Registration number:
This declaration is based on Product Category Rules: NEPD-8428-8099-EN
CEN Standard EN 15804:2012+A2:2019 serves as core
Issue date: 10.12.2024
PCR.
The Norwegian EPD Foundation NPCR 012:2022 Part B for Thermal insulation products Valid to: 10.12.2029
EPD software:
LCAno EPD generator ID: 643679
1 / 11
General information
Product Owner of the declaration:
Sto-InnoDrain Sto SE & Co. KGaA
Contact person: Linus Kaltenbach
Phone: +49 7744571010
e-mail: infoservice@sto.com
Program operator: Manufacturer:
The Norwegian EPD Foundation Sto Scandinavia AB
Post Box 5250 Majorstuen, 0303 Oslo, Norway Gesällgatan 6
Phone: +47 977 22 020 SE-582 77 Linköping, Sweden
web: www.epd-norge.no
Declaration number: Place of production:
Linköping
NEPD-8428-8099-EN Gesällgatan 6
SE-582 77 Linköping, Sweden
This declaration is based on Product Category Rules: Management system:
CEN Standard EN 15804:2012+A2:2019 serves as core PCR. ISO 14001; ISO 50001; ISO 9001
NPCR 012:2022 Part B for Thermal insulation products
Statement of liability: Organisation no:
The owner of the declaration shall be liable for the underlying DE142834082
information and evidence. EPD Norway shall not be liable with respect
to manufacturer information, life cycle assessment data and
evidences.​
Declared unit: Issue date:
1 m2 Sto-InnoDrain
10.12.2024
Declared unit with option: Valid to:
A1,A2,A3,A4,A5,C1,C2,C3,C4,D 10.12.2029
Year of study:
2023
Functional unit: Comparability:
1 m² with 33 mm thickness at R=1 m²K/W. Weight per declared unit EPD of construction products may not be comparable if they not
is 0,759 kg at density 23 kg/m³ and thickness 33 mm. comply with EN 15804:2012+A2:2019 and seen in a building context.
General information on verification of EPD from EPD tools: Development and verification of EPD:
Independent verification of data, other environmental information The declaration is created using EPD tool lca.tools ver EPD2022.03,
and the declaration according to ISO 14025:2010, § 8.1.3 and § 8.1.4. developed by LCA.no. The EPD tool is integrated in the company's
Verification of each EPD is made according to EPD-Norway’s management system, and has been approved by EPD Norway.
guidelines for verification and approval requiring that tools are i) NEPDT143
integrated into the company's environmental management system, ii)
the procedures for use of the EPD tool are approved by EPD-Norway, Developer of EPD: Karin Bromoe
and iii) the process is reviewed annually by an independent third
Reviewer of company-specific input data and EPD:​ Angelica Hultin
party verifier. See Appendix G of EPD-Norway's General Programme
Instructions for further information on EPD tools
Verification of EPD tool: Approved:
Independent third party verification of the EPD tool, background data
and test-EPD in accordance with EPDNorway's procedures and
guidelines for verification and approval of EPD tools.
Håkon Hauan, CEO EPD-Norge
Third party verifier:
Elisabet Amat, GREENIZE projects
(no signature required)
2 / 11
Product
Product description:
Sto-InnoDrain is an insulation board of expanded polystyrene according to EN 13163 with a drainage effect.
Sto-InnoDrain is used as a facade insulation board intended for outdoor use, in StoTherm Vario D or in other StoTherm facade systems exposed to
moisture. The board should be glued or plugged and glued on the facade.
Sto-InnoDrain is manufactured by heating polystyrene grains, containing approximately 5% pentane, with steam. The polystyrene grains expand
until they contain 98% of air. The pre-expanded polystyrene will first be dried, before mixing with additional materials. The EPS-mixture is
thereafter dried and moulded under compression. After the stabilization phase, the products are ready for packaging and labelling. Sto-InnoDrain
boards which don't pass the quality control at the production site, are recycled into new Sto-InnoDrain boards.
Sto-InnoDrain is provided in several thicknesses. The average density of Sto-InnoDrain boards with thickness between 30 mm - 200 mm is
approximately 23 kg/m³.
Weight per declared unit is 0,759 kg with density of 23 kg/m³ and thickness of 33 mm.
Please use the conversion table in this EPD, page 4, for other thicknesses then the declared unit.
Product specification
Materials Value Unit
Expanded polystyrene < 70 %
Binders 10-25 %
Additive 10-25 %
Packaging 0.5-3 %
Technical data:
Thermal conductivity = 0,033 W/(m*K)
Fire class: E according to EN 13501-1
Format: 120 x 60 cm
Typical thickness: 30 mm - 200 mm
Market:
Germany, Sweden, Norway and Finland.
Reference service life, product
If applied correctly, the lifetime of EPS insulation is equal to building life time without requiring maintenance.
Reference service life, building or construction works
The reference service life of the building is set to be minimum 60 years in this EPD.
LCA: Calculation rules
Declared unit:
1 m2 Sto-InnoDrain
Cut-off criteria:
All major raw materials and all the essential energy is included. The production processes for raw materials and energy flows with very small
amounts (less than 1%) are not included. These cut-off criteria do not apply for hazardous materials and substances.
Allocation:
The allocation is made in accordance with the provisions of EN 15804+A2. Incoming energy and water and waste production in-house is allocated
equally among all products through mass allocation. Effects of primary production of recycled materials is allocated to the main product in which
the material was used. The recycling process and transportation of the material is allocated to this analysis.
Data quality:
Specific data for the product composition are provided by the manufacturer. The data represent the production of the declared product and were
collected for EPD development in the year of study. Background data is based on EPDs according to EN 15804 and different LCA databases. The
data quality of the raw materials in A1 is presented in the table below.
Materials Source Data quality Year
Binders and Resins ecoinvent 3.6 Database 2019
Chemical ecoinvent 3.6 Database 2019
Packaging - Plastic ecoinvent 3.6 Database 2019
Packaging - Polystyrene ecoinvent 3.6 Database 2019
European
Plastic - Polystyrene expandable (EPS) Plastics Europe + ecoinvent 3.6 2019
average.
3 / 11
System boundaries (X=included, MND=module not declared, MNR=module not relevant)
Construction Beyond the system
Product stage Use stage End of life stage
installation stage boundaries
A1 A2 A3 A4 A5 B1 B2 B3 B4 B5 B6 B7 C1 C2 C3 C4 D
X X X X X MND MND MND MND MND MND MND X X X X X
System boundary:
The approach is “cradle-to-grave” but with exclusion of the use stage (B1-B7). Stage B1-B7 is not applicable for this thermal insulation product.
Sto-InnoDrain does not require any actions or maintenance operations during the use stages. The following modules have been considered:
A1, A2, A3 (Product stages): Extraction and transport of raw materials, including packaging, and manufacturing process
A4 (Transport to market): Transportation from manufacturing plant to customer
A5 (Assembly): Installation at construction site
C1, C2, C3, C4 (End of life stages): Deconstruction, demolition, transport to waste processing, waste processing for reuse, recovery and/or recycling
and disposal
D (Benefits and loads beyond the system boundaries): Reuse/recovery/recycling potential
Additional technical information:
The waste key for unused product is 17 06 04 Insulation material other than those covered by 17 06 01 och 17 06 03.
waR slairetam tropsnarT gnirutcafunaM tropsnarT ylbmessA e​sU ecnanetniaM riapeR tnemecalpeR tnemhsibrufeR lanoitarepO ygrene esu lanoitarepO esu retaw -eD noitcurtsnoc noitilomed tropsnarT etsaW gnissecorp lasopsiD -yrevoceR-esueR laitnetop-gnilcyceR
4 / 11
LCA: Scenarios and additional technical information
The following information describe the scenarios in the different modules of the EPD.
A4 (Transport to market/building site): An average distance is calculated based on the production site in Linköping and transport to customers in
Stockholm and Stühlingen in Germany. The average distance is 200 km by (Truck 16-32 tonnes), 1418 km by (Truck 16-32 tonnes) HVO100 and
Ferry 153 km. About 50% of all produced Sto-InnoDrain is sold to Germany. This has been taken into account in the LCA calculation.
A5 (Installation): The product is applied according to the specification in the technical data sheet at the building site. Installation is generally done
manually. Electricity for applying screws with drilling machine when applying the board with plug has not been taken into account in this LCA.
Outputs are small amounts of waste from the product itself (assumed to be less than 3%) and waste from packaging materials.
C1 (De-construction, demolition): In this LCA it is assumed that Sto-InnoDrain is dismantled manually.
C2 (Transport end of life): This stage includes the transportation effects of demolished waste to a waste processing area. The distance between the
demolishing area and a waste processing area is assumed to be quite short (less than 100 km).
C3, C4 (Waste processing): The insulation board is not classified as hazardous waste. In this LCA we have assumed a typical waste scenario that is
incineration.
D (Environmental costs and benefits of recycling and reuse): Energy credit related to energy recovery from the incineration is included in module
D.
Stages not included:
Once installation is complete, no actions or technical operations are required during the use stage until the end of life stage. Stages B1-B7 are
therefore not included.
Capacity utilisation Value
Transport from production place to user (A4) Distance (km) Fuel/Energy Consumption Unit
(incl. return) % (Liter/tonne)
Ship, Ferry, Sea (kgkm) 50,0 % 153 0,034 l/tkm 5,20
Truck, 16-32 tonnes, EURO 6 (kgkm) 36,7 % 200 0,043 l/tkm 8,60
Truck, 16-32 tonnes, HVO, EURO 6 (kgkm) - RER 36,7 % 1418 0,043 l/tkm 60,97
Assembly (A5) Unit Value
Material loss, including waste treatment (psc) Units/DU 0,02
Waste, packaging, polystyrene, for incineration
kg 0,00
(kg)
Waste, packaging, plastic film (LDPE), to average
kg 0,01
treatment (kg)
Capacity utilisation Value
Transport to waste processing (C2) Distance (km) Fuel/Energy Consumption Unit
(incl. return) % (Liter/tonne)
Truck, 16-32 tonnes, EURO 6 (kgkm) 36,7 % 100 0,043 l/tkm 4,30
Waste processing (C3) Unit Value
Waste treatment per kg Expanded Polystyrene
kg/DU 0,76
(EPS), incineration - C3 (kg)
Disposal (C4) Unit Value
Landfilling of ashes from incineration of
expanded polystyrene (EPS), process per kg ashes kg 0,03
and residues (kg)
Benefits and loads beyond the system
Unit Value
boundaries (D)
Substitution of electricity, in Norway (MJ) MJ 0,00
Substitution of thermal energy, district heating, in
MJ 0,07
Norway (MJ)
Substitution of electricity (MJ) MJ 0,00
Substitution of thermal energy, district heating
MJ 0,00
(MJ)
Substitution of thermal energy, district heating
MJ 17,47
(MJ)
Substitution of electricity (MJ) MJ 1,15
5 / 11
LCA: Results
The LCA results are presented below for the declared unit defined on page 2 of the EPD document.
Environmental impact
Indicator Unit A1 A2 A3 A4 A5 C1 C2 C3 C4 D
GWP-total
kg CO2 -
1,92E+00 9,37E-02 1,56E-01 4,02E-02 8,79E-03 0 1,26E-02 2,41E+00 1,73E-03 -1,05E-01
eq
GWP-fossil
kg CO2 -
1,91E+00 9,36E-02 1,54E-01 4,01E-02 8,79E-03 0 1,25E-02 2,41E+00 1,73E-03 -1,02E-01
eq
GWP-biogenic
kg CO2 -
7,79E-03 4,16E-05 6,29E-04 4,26E-05 1,28E-07 0 5,19E-06 2,22E-05 8,98E-07 -2,10E-04
eq
GWP-luluc
kg CO2 -
7,48E-04 3,32E-05 1,63E-03 4,14E-05 4,80E-08 0 4,46E-06 3,14E-06 2,53E-07 -3,50E-03
eq
kg
ODP CFC11 - 3,62E-08 2,23E-08 1,30E-08 8,49E-09 3,60E-11 0 2,84E-09 1,90E-09 1,69E-10 -7,41E-03
eq
mol H+
AP 5,06E-03 5,37E-04 2,28E-04 3,96E-04 1,62E-06 0 3,60E-05 2,89E-04 5,79E-06 -8,38E-04
-eq
EP-FreshWater kg P -eq 1,54E-05 7,74E-07 2,39E-06 9,00E-07 1,67E-09 0 1,00E-07 1,92E-07 2,36E-08 -9,04E-06
EP-Marine kg N -eq 1,02E-03 1,26E-04 4,28E-05 9,91E-05 1,04E-06 0 7,13E-06 1,38E-04 1,78E-06 -2,74E-04
mol N -
EP-Terrestial 1,19E-02 1,41E-03 5,33E-04 1,10E-03 7,34E-06 0 7,98E-05 1,48E-03 2,03E-05 -2,96E-03
eq
kg
POCP NMVOC 4,13E-03 4,59E-04 1,91E-02 3,42E-04 1,96E-06 0 3,06E-05 3,55E-04 5,59E-06 -8,17E-04
-eq
ADP- kg Sb-
3,33E-05 1,72E-06 1,24E-06 2,96E-06 2,94E-09 0 3,46E-07 9,14E-08 8,72E-09 -1,01E-06
minerals&metals1 eq
ADP-fossil1 MJ 5,45E+01 1,51E+00 3,07E+00 7,19E-01 2,61E-03 0 1,90E-01 1,56E-01 1,46E-02 -1,45E+00
WDP1 m3 9,72E+00 1,18E+00 2,98E+02 1,52E+00 8,82E-03 0 1,83E-01 4,65E-01 1,67E-01 -1,81E+01
GWP-total = Global Warming Potential total; GWP-fossil = Global Warming Potential fossil fuels; GWP-biogenic = Global Warming Potential biogenic; GWP-luluc =
Global Warming Potential land use and land use change; ODP = Depletion potential of the stratospheric ozone layer; AP = Acidification potential, Accumulated
Exceedance; EP-freshwater = Eutrophication potential, fraction of nutrients reaching freshwater end compartment: EP-marine = Eutrophication potential, fraction of
nutrients reaching marine end compartment; EP-terrestrial = Eutrophication potential, Accumulated Exceedance; POCP = Formation potential of tropospheric ozone;
ADP-minerals&metals = Abiotic depletion potential for non-fossil resources; ADP-fossil = Abiotic depletion for fossil resources potential; WDP = Water (user)
deprivation potential, deprivation-weighted water consumption
"Reading example: 9,0 E-03 = 9,0*10-3 = 0,009"
*INA Indicator Not Assessed
1. The results of this environmental impact indicator shall be used with care as the uncertainties on these results are high or as there is limited experienced with the
indicator
Remarks to environmental impacts
6 / 11
Additional environmental impact indicators
Indicator Unit A1 A2 A3 A4 A5 C1 C2 C3 C4 D
PM Disease incidence 3,87E-08 8,60E-09 1,67E-09 5,84E-09 1,50E-11 0 7,68E-10 1,23E-09 6,80E-11 -5,08E-08
IRP2 kgBq U235 -eq 5,43E-02 6,54E-03 1,01E-01 2,64E-03 1,03E-05 0 8,29E-04 2,85E-04 7,06E-05 -9,29E-03
ETP-fw1 CTUe 2,14E+02 1,12E+00 1,72E+00 8,40E-01 3,26E-03 0 1,41E-01 3,72E-01 2,92E-02 -7,91E+00
HTP-c1 CTUh 8,22E-10 0,00E+00 7,50E-11 0,00E+00 0,00E+00 0 0,00E+00 1,02E-10 1,00E-12 -1,44E-10
HTP-nc1 CTUh 2,84E-08 1,14E-09 1,81E-09 1,30E-09 1,60E-11 0 1,54E-10 4,03E-09 5,50E-11 -7,58E-09
SQP1 dimensionless 2,74E+00 1,72E+00 1,33E+00 9,76E-01 3,76E-03 0 1,33E-01 2,03E-02 4,03E-02 -9,72E+00
PM = Particulate Matter emissions; IRP = Ionizing radiation – human health; ETP-fw = Eco toxicity – freshwater; HTP-c = Human toxicity – cancer effects; HTP-nc =
Human toxicity – non cancer effects; SQP = Potential Soil Quality Index (dimensionless)
"Reading example: 9,0 E-03 = 9,0*10-3 = 0,009"
*INA Indicator Not Assessed
1. The results of this environmental impact indicator shall be used with care as the uncertainties on these results are high or as there is limited experienced with the
indicator
2. This impact category deals mainly with the eventual impact of low dose ionizing radiation on human health of the nuclear fuel cycle. It does not consider effects due
to possible nuclear accidents, occupational exposure nor due to radioactive waste disposal in underground facilities. Potential ionizing radiation from the soil, from
radon and from some construction materials is also not measured by this indicator.
7 / 11
Resource use
Indicator Unit A1 A2 A3 A4 A5 C1 C2 C3 C4 D
PERE MJ 5,61E-01 1,97E-02 1,42E+00 2,35E-02 6,89E-05 0 2,71E-03 5,22E-03 9,25E-04 -8,98E+00
PERM MJ 0,00E+00 0,00E+00 0,00E+00 0,00E+00 0,00E+00 0 0,00E+00 0,00E+00 0,00E+00 0,00E+00
PERT MJ 5,61E-01 1,97E-02 1,42E+00 2,35E-02 6,89E-05 0 2,71E-03 5,22E-03 9,25E-04 -8,98E+00
PENRE MJ 3,38E+01 1,51E+00 3,07E+00 7,19E-01 2,61E-03 0 1,90E-01 1,56E-01 1,46E-02 -1,45E+00
PENRM MJ 2,22E+01 0,00E+00 0,00E+00 0,00E+00 -3,68E-01 0 0,00E+00 -2,18E+01 0,00E+00 0,00E+00
PENRT MJ 5,60E+01 1,51E+00 3,07E+00 7,19E-01 -3,65E-01 0 1,90E-01 -2,17E+01 1,46E-02 -1,45E+00
SM kg 1,37E-03 0,00E+00 8,36E-05 0,00E+00 0,00E+00 0 0,00E+00 0,00E+00 0,00E+00 0,00E+00
RSF MJ 1,19E-02 6,76E-04 7,06E-03 7,68E-04 1,83E-06 0 9,71E-05 1,46E-04 2,29E-05 -1,57E-03
NRSF MJ 8,59E-04 2,20E-03 1,88E-02 2,61E-03 8,24E-06 0 3,47E-04 0,00E+00 2,72E-03 -5,33E-01
FW m3 4,51E-02 1,80E-04 2,90E-02 2,07E-04 2,56E-06 0 2,03E-05 6,99E-04 1,34E-05 -1,08E-02
PERE = Use of renewable primary energy excluding renewable primary energy resources used as raw materials; PERM = Use of renewable primary energy resources used
as raw materials; PERT = Total use of renewable primary energy resources; PENRE = Use of non renewable primary energy excluding non-renewable primary energy
resources used as raw materials; PENRM = Use of non renewable primary energy resources used as raw materials; PENRT = Total use of non renewable primary energy
resources; SM = Use of secondary materials; RSF = Use of renewable secondary fuels; NRSF = Use of non-renewable secondary fuels; FW = Net use of fresh water
"Reading example: 9,0 E-03 = 9,0*10-3 = 0,009"
*INA Indicator Not Assessed
8 / 11
End of life - Waste
Indicator Unit A1 A2 A3 A4 A5 C1 C2 C3 C4 D
HWD kg 3,33E-03 8,56E-05 1,32E-03 7,58E-05 0,00E+00 0 9,78E-06 0,00E+00 2,26E-02 -6,84E-05
NHWD kg 7,81E-02 1,31E-01 1,24E-02 7,59E-02 8,90E-03 0 9,22E-03 0,00E+00 1,48E-02 -3,44E-02
RWD kg 1,25E-05 1,02E-05 4,47E-05 3,66E-06 0,00E+00 0 1,29E-06 0,00E+00 8,77E-08 -7,61E-06
HWD = Hazardous waste disposed; NHWD = Non-hazardous waste disposed; RWD = Radioactive waste disposed
"Reading example: 9,0 E-03 = 9,0*10-3 = 0,009"
*INA Indicator Not Assessed
End of life - Output flow
Indicator Unit A1 A2 A3 A4 A5 C1 C2 C3 C4 D
CRU kg 0,00E+00 0,00E+00 0,00E+00 0,00E+00 0,00E+00 0 0,00E+00 0,00E+00 0,00E+00 0,00E+00
MFR kg 0,00E+00 0,00E+00 2,68E-03 0,00E+00 3,22E-03 0 0,00E+00 0,00E+00 0,00E+00 0,00E+00
MER kg 0,00E+00 0,00E+00 4,15E-04 0,00E+00 2,60E-03 0 0,00E+00 7,59E-01 0,00E+00 0,00E+00
EEE MJ 0,00E+00 0,00E+00 5,81E-02 0,00E+00 4,58E-03 0 0,00E+00 1,15E+00 0,00E+00 0,00E+00
EET MJ 0,00E+00 0,00E+00 8,79E-01 0,00E+00 6,93E-02 0 0,00E+00 1,75E+01 0,00E+00 0,00E+00
CRU = Components for re-use; MFR = Materials for recycling; MER = Materials for energy recovery; EEE = Exported energy electrical; EET = Exported energy thermal
"Reading example: 9,0 E-03 = 9,0*10-3 = 0,009"
*INA Indicator Not Assessed
Biogenic Carbon Content
Indicator Unit At the factory gate
Biogenic carbon content in product kg C 0,00E+00
Biogenic carbon content in accompanying packaging kg C 0,00E+00
Note: 1 kg biogenic carbon is equivalent to 44/12 kg CO2
9 / 11
Additional requirements
Greenhouse gas emissions from the use of electricity in the manufacturing phase
National production mix from import, low voltage (production of transmission lines, in addition to direct emissions and losses in grid) of applied
electricity for the manufacturing process (A3).
Electricity mix Source Amount Unit
Electricity, Sweden (kWh) ecoinvent 3.6 54,94 g CO2-eq/kWh
Dangerous substances
The product contains no substances given by the REACH Candidate list.
Indoor environment
Not relevant.
Additional Environmental Information
Additional environmental impact indicators required in NPCR Part A for construction products
Indicator Unit A1 A2 A3 A4 A5 C1 C2 C3 C4 D
GWPIOBC kg CO2 -eq 1,91E+00 9,37E-02 1,56E-01 4,02E-02 8,79E-03 0 1,26E-02 2,41E+00 1,80E-03 -1,04E-01
GWP-IOBC: Global warming potential calculated according to the principle of instantaneous oxidation. In order to increase the transparency of biogenic carbon​
contribution to climate impact, the indicator GWP-IOBC is required as it declares climate impacts calculated according to the principle of instantaneous oxidation.​
GWP-IOBC is also referred to as GWP-GHG in context to Swedish public procurement legislation.
10 / 11
Bibliography
ISO 14025:2010 Environmental labels and declarations - Type III environmental declarations - Principles and procedures.
ISO 14044:2006 Environmental management - Life cycle assessment - Requirements and guidelines.
EN 15804:2012+A2:2019 Environmental product declaration - Core rules for the product category of construction products.
ISO 21930:2017 Sustainability in buildings and civil engineering works - Core rules for environmental product declarations of construction
products.
ecoinvent v3, Allocation, cut-off by classification, Swiss Centre of Life Cycle Inventories.
Iversen et al., (2021) eEPD v2021.09 Background information for EPD generator tool system verification, LCA.no Report number: 07.21
Vold et. al., (2022) EPD generator for NPCR 012 Thermal insulation, Background information for EPD generator application and LCA data, LCA.no
report number: 07.22.
NPCR Part A: Construction products and services. Ver. 2.0. April 2021, EPD-Norge.
NPCR 012 Part B for Part B for Thermal insulation products, Ver. 2.0, 31.03.2022, EPD Norway.
Program operator and publisher Phone: +47 977 22 020
The Norwegian EPD Foundation e-mail: post@epd-norge.no
Post Box 5250 Majorstuen, 0303 Oslo, Norway web: www.epd-norge.no
Owner of the declaration: Phone: +49 7744571010
Sto SE & Co. KGaA e-mail: infoservice@sto.com
Ehrenbachstraße 1, 79780 Stühlingen, Germany web: https://www.sto.com/
Author of the Life Cycle Assessment Phone: +47 916 50 916
LCA.no AS e-mail: post@lca.no
Dokka 6A, 1671 Kråkerøy, Norway web: www.lca.no
Developer of EPD generator Phone: +47 916 50 916
LCA.no AS e-mail: post@lca.no
Dokka 6A, 1671 Kråkerøy, Norway web: www.lca.no
ECO Platform web: www.eco-platform.org
ECO Portal web: ECO Portal
11 / 11
