ENVIRONMENTAL PRODUCT DECLARATION
as per /ISO 14025/ and /EN 15804/
Owner of the Declaration Türk Ytong Sanayi A.Ş.
Programme holder Institut Bauen und Umwelt e.V. (IBU)
Publisher Institut Bauen und Umwelt e.V. (IBU)
Declaration number EPD-TYS-20180105-CAD1-EN
Issue date 09.03.2020
Valid to 08.03.2025
Ytong® Autoclaved Aerated Concrete Block and AAC
Blocks for Floor Plates
Türk Ytong Sanayi A.Ş.
www.ibu-epd.com / https://epd-online.com
Umwelt Produktdeklaration Name des Herstellers – Name des Produkts
General Information
Türk Ytong Sanayi A.Ş. Autoclaved Aerated Concrete (AAC)
Block and AAC Blocks for Floor
Plates
Programme holder Owner of the Declaration
IBU - Institut Bauen und Umwelt e.V. Türk Ytong Sanayi A.Ş.
Panoramastr. 1
10178 Berlin Headquarters
Germany Aydınevler Mahallesi, İnönü Caddesi, Gökçe Sokak
34854 No:3 Maltepe İstanbul Turkey
Declaration number Declared product / Declared unit
EPD-TYS-20180105-CAD1-EN 1 m3 AAC block and AAC Blocks for Floor Plates with
an average gross density of 388 kg/m3
This Declaration is based on the Product Scope:
Category Rules: This EPD and its LCA are relevant to AAC blocks and
Aerated concrete, 07.2014 AAC Blocks for Floor Plates produced in the plants of
(PCR tested and approved by the SVR) TURK YTONG located in Antalya, Bilecik, Çatalca
(Istanbul), Pendik (Istanbul) and Saray (Trakya),
Turkey. The calculations are based on average
Issue date
production data collected during the year 2016 (from
09.03.2020
January to December). A weighted average was
calculated as an annual representative value (12
Valid to months).
08.03.2025
The owner of the declaration shall be liable for the
underlying information and evidence; the IBU shall not
be liable with respect to manufacturer information, life
cycle assessment data and evidences.
Verification
The CEN Norm /EN 15804/ serves as the core PCR
Independent verification of the declaration
according to /ISO 14025/
Dipl. Ing. Hans Peters internally x externally
(President of Institut Bauen und Umwelt e.V.)
Dr. Alexander Röder Prof. Dr. Birgit Grahl
(Managing Director IBU) (Independent verifier appointed by SVR)
Product
Product description / Product definition of walling including single leaf, cavity, partitions,
The products mentioned are AAC blocks and AAC retaining, basement and general use below ground
Blocks for Floor Plates in various formats made of level, including walling for fire protection, thermal
autoclaved aerated concrete. AAC belongs to the insulation, sound insulation and the fabric of chimneys
porous steam-cured light-weight concrete group. (excluding chimney flue units). AAC blocks for floor
plates are used as infills in cast-in-situ infilled joist floor
For the placing on the market of the product in the systems
EU/EFTA (with the exception of Switzerland)
Regulation (EU) No. 305/2011 (CPR) applies. The
product needs a Declaration of Performance taking Technical Data
into consideration /EN 771-4:2015-11/, Specification AAC blocks and AAC blocks for floor plates
for masonry units - Part 4: Autoclaved aerated demonstrate the following constructional performance:
concrete masonry units/ and the CE-Marking. For the
application and use the respective national provisions Constructional data
apply. Name Value Unit
Compressive strength acc. to /TS
1.5 - 5 N/mm2
EN 772-1/
Application Tensile strength acc. to /TS EN
0.24 - 1 N/mm2
AAC blocks are used to form different types of load 1351/
bearing and nonload bearing applications in all forms Modulus of elasticity acc. to /TS 750 - 2250 N/mm2
2 Environmental Product Declaration TÜRK YTONG SANAYİ A.Ş. – AAC block and AAC Blocks for Floor Plates
EN 1352/ materials (slurry and powder are recycled 100% in a
Thermal conductivity acc. to /TS 0.085 - closed loop) that has been reduced to small pieces,
W/(mK)
EN 12664/ 0.16 adding water and aluminum powder, in a mixer, until it
Moisture content at 23 °C, 80% 4 M.-% becomes a slurry. It is then poured into a casting
Shrinkage acc. to /TS EN 680/ 0.2 mm/m mould. The aluminum reacts in an alkaline milieu.
Water vapour diffusion coefficient Thus, gaseous hydrogen is formed which creates
acc. to /TS EN 1745/ 5/10 pores in the mass and escapes without leaving any
Cross dry density acc. to /TS EN residue. The pores usually have a diameter of (0.5-1.5
300 - 600 kg/m³ mm) and are filled exclusively with air. After setting
772-13/
once, semisolid raw blocks are created, from which the
autoclaved aerated concrete building components are
then cut with high precision.
The formation of the final qualities of the building
component occurs during the subsequent steam-curing
Base materials / Ancillary materials
over 5-12 hours at approximately 190° C with
 Portland Cement 15-30%
approximately 12 bar pressure in steam pressure
 Quicklime 10-20%
kettles or autoclaves, as they are called. The used
 Quartzite/Sand 50-70%
substances create calcium hydro silicates, which
 Gypsum 2-5% corresponds to the naturally occurring mineral
 Aluminium 0.05-0.1% tobermorite. The reaction of the material is complete
when removed from the autoclave. Therefore, the
reaction does not take as long as the hardening of
concrete. Once the steaming process is complete, the
In addition, 40-60% water is used (based on the solid
steam is used for other autoclave cycles. Thereby,
materials).
energy is saved and harm to the environment due to
hot exhaust steam and wastewater is avoided.
The ground quartzite is mixed with gypsum, cement
produced according to /TS EN 197-1/, quicklime in
The production process is shown in the following
accordance with /TS EN 459-1/ and AAC recycling
figure:
According to the Sustainable Building Guideline of IBU
the average life expectancy of AAC is 100 years.
Reference service life Further Information
In this study, Reference Service Life (RSL) is not taken For further information, please contact Türk Ytong A.S.
into consideration during the calculations since the through its website at www.ytong.com.tr
system boundary of this EPD is cradle-to-gate.
AAC does not change once it leaves the autoclaves.
When used as intended, it is boundlessly stable.
3 Environmental Product Declaration TÜRK YTONG SANAYİ A.Ş. – AAC block and AAC Blocks for Floor Plates
LCA: Calculation rules
Declared Unit floor plates products from extraction of raw material to
The declared unit is defined as 1m3 of AAC block and the production of finished packed product at the plant
AAC block for floor plates group. This declaration is gate.
classified as an average product as calculated from the
overall production in several of the manufacturer’s The product stage contains A1 (extraction, processing,
plants as 1d according to PCR Part A. production of raw materials), A2 (Transport to the
manufacturer and internal transport) and A3
Declared unit (Manufacturing operations) modules. These are
Name Value Unit declared separately.
Declared unit 1 m3
Conversion factor to 1 kg 0.002577 - Background data
Gross dry density 388 kg/m³ All relevant background datasets were taken from the
/Ecoinvent/ database within /SimaPro/ software.
System boundary
Type of the EPD: cradle-to-gate Comparability
Basically, a comparison or an evaluation of EPD data
The system boundaries of this life cycle assessment is only possible if all the data sets to be compared
study are considered as cradle-to-gate, since all the were created according to /EN 15804/ and the building
modules except A1-A3 product stage are not declared context, respectively the product-specific
within the scope of this study. This means the system characteristics of performance, are taken into account.
boundary covers Ytong AAC block and AAC block for .
LCA: Scenarios and additional technical information
A1, A2 and A3 modules are declared within the scope
of this study. Hence, there are no scenarios provided
below regarding the other modules A4, A5, B1-B7, C1-
C4 and D.
In this study, closed-loop recycling was used. Ytong
plants utilize recycled waste (slurry and powder)
internally.
Type and amount of packaging materials:
A weighted average value of five plants of packaging
materials used for 1m3 AAC Blocks is PE strech film
(0.580kg), wooden pallet (0.881 piece), PE etiquette
(0.000893kg) and ink(0.000449kg).
4 Environmental Product Declaration TÜRK YTONG SANAYİ A.Ş. – AAC block and AAC Blocks for Floor Plates
LCA: Results
The following table shows the impact estimate results which are relative expressions and do not predict impacts
on category endpoints or the transgression of thresholds, safety margins or risks.
DESCRIPTION OF THE SYSTEM BOUNDARY (X = INCLUDED IN LCA; MND = MODULE NOT DECLARED)
BENEFITS AND
CONSTRUCTI LOADS
PRODUCT STAGE ON PROCESS USE STAGE END OF LIFE STAGE BEYOND THE
STAGE SYSTEM
BOUNDARIES
5 Environmental Product Declaration TÜRK YTONG SANAYİ A.Ş. – AAC block and AAC Blocks for Floor Plates
lairetam
waR
ylppus tropsnarT
gnirutcafunaM
eht
morf
tropsnarT
etis
eht
ot
etag
ylbmessA esU
ecnanetniaM
riapeR
tnemecalpeR tnemhsibrufeR
ygrene
lanoitarepO esu
retaw
lanoitarepO esu
noitcurtsnoc-eD
noitilomed tropsnarT
gnissecorp
etsaW
lasopsiD -esueR -yrevoceR -gnilcyceR laitnetop
A1 A2 A3 A4 A5 B1 B2 B3 B4 B5 B6 B7 C1 C2 C3 C4 D
X X X MND MND MND MND MNR MNR MNR MND MND MND MND MND MND MND
RESULTS OF THE LCA - ENVIRONMENTAL IMPACT: 1 m3 AAC block and AAC block for floor plates
Parameter Unit A1 A2 A3
Global warming potential [kg CO2-Eq.] 1.40E+2 6.59E+0 2.49E+1
Depletion potential of the stratospheric ozone layer [kg CFC11-Eq.] 5.77E-6 1.24E-6 1.38E-6
Acidification potential of land and water [kg SO2-Eq.] 2.99E-1 3.30E-2 1.01E-1
Eutrophication potential [kg (PO4)3--Eq.] 3.73E-2 6.21E-3 5.85E-3
Formation potential of tropospheric ozone photochemical oxidants [kg ethene-Eq.] 2.03E-2 1.18E-3 4.79E-3
Abiotic depletion potential for non-fossil resources [kg Sb-Eq.] 1.16E-3 1.39E-5 6.15E-6
Abiotic depletion potential for fossil resources [MJ] 7.36E+2 9.89E+1 3.56E+2
RESULTS OF THE LCA - RESOURCE USE: 1 m3 AAC block and AAC block for floor plates
Parameter Unit A1 A2 A3
Renewable primary energy as energy carrier [MJ] 4.61E+2 1.24E+0 1.76E+1
Renewable primary energy resources as material utilization [MJ] 1.04E+2 IND IND
Total use of renewable primary energy resources [MJ] 5.65E+2 1.24E+0 1.76E+1
Non-renewable primary energy as energy carrier [MJ] 7.39E+2 1.01E+2 3.59E+2
Non-renewable primary energy as material utilization [MJ] 2.53E+1 IND IND
Total use of non-renewable primary energy resources [MJ] 7.65E+2 1.01E+2 3.59E+2
Use of secondary material [kg] IND IND IND
Use of renewable secondary fuels [MJ] IND IND IND
Use of non-renewable secondary fuels [MJ] IND IND IND
Use of net fresh water [m³] 9.01E-3 1.75E-3 4.03E-1
RESULTS OF THE LCA – OUTPUT FLOWS AND WASTE CATEGORIES:
1 m3 AAC block and AAC block for floor plates
Parameter Unit A1 A2 A3
Hazardous waste disposed [kg] 1.58E-3 5.12E-5 1.93E-4
Non-hazardous waste disposed [kg] 3.32E+0 3.69E+0 5.56E-1
Radioactive waste disposed [kg] 3.18E-3 7.08E-4 8.31E-5
Components for re-use [kg] IND IND IND
Materials for recycling [kg] IND IND IND
Materials for energy recovery [kg] IND IND IND
Exported electrical energy [MJ] IND IND IND
Exported thermal energy [MJ] IND IND IND
Note: There are no direct radioactive wastes during the manufacturing processes. In the manufacturing stage (A3), the value acquired for radioactive waste generation mostly
is in relation with the upstream processes of electricity and natural gas, respectively.
Requisite evidence
Radioactivity
All mineral raw materials contain small amounts of naturally radioactive substances. The measurements show
that the natural radioactivity from a radiological point of view allows an unrestricted use of this building material.
References
SimaPro LCA Package, Pré Consultants, the
Institut Bauen und Umwelt Netherlands, www.pre-sustainability.com (v8.3.0.0)
Institut Bauen und Umwelt e.V., Berlin (pub.):
Generation of Environmental Product Declarations
(EPDs); /TS EN 197-1/
General Principles Cement - Part 1: Composition, specifications and
for the EPD range of Institut Bauen und Umwelt e.V. conformity criteria for common cements
(IBU), 2015/10
www.ibu-epd.de /TS EN 459-1/
Building lime - Part 1: Definitions, specifications and
/ISO 14025/ conformity criteria
DIN EN /ISO 14025:2011-10/, Environmental labels
and declarations — Type III environmental
declarations — Principles and procedures /TS EN 680/
Determination of the drying shrinkage of autoclaved
/EN 15804/ aerated concrete
/EN 15804:2012-04+A1 2013/, Sustainability of
construction works — Environmental Product /TS EN 771-4/
Declarations — Core rules for the product category of Specification for masonry units - Part 4: Autoclaved
construction products aerated concrete masonry units
/PCR Part A/ /TS EN 12664/
Product Category Rules for Building Related Products Thermal performance of building materials and
and Services , Institute Construction and Environment products - Determination of thermal resistance by
e.V. (IBU) Part A: Calculation Rules for the Life Cycle means of guarded hot plate and heat flow meter
Assessment and Requirements on the Project Report methods - Dry and moist products of medium and low
(version 1.6),11.04.2017; www.bau-umwelt.de thermal resistance
/PCR Part B/ /TS EN 1745/
Masonry and masonry products - Methods for
Product Category Rules (PCR), Guidance-Texts for determining thermal properties
Building-Related Products and Services, from the
range of Environmental Product Declarations of /CPR/
Institute Construction and Environment e.V. (IBU), Part No305/211 Construction Products Regulation
B: Requirements on the EPD for Aerated concrete,
version 1.3, 04.07.2014 /TS EN 772-1/
www.bau-umwelt.de Determination of compressive strength
/TS EN 772-13/
/ISO 14040-44/ Determination of net and gross dry density of
DIN EN ISO 14040:2006: Environmental management masonry units (except for natural stone)
- Life cycle assessment - Principles and framework
(ISO 14040:2006) and Requirements and guidelines /TS EN 1352/
(ISO 14044:2006) Determination of static modulus of elasticity under
compression of autoclaved aerated concrete or
/Ecoinvent/ lightweight aggregate concrete with open structure
Ecoinvent Centre, www.ecoinvent.com (v3.3)
/TS EN 1351/
/SimaPro/ Determination of flexural strength of autoclaved
aerated concrete
6 Environmental Product Declaration TÜRK YTONG SANAYİ A.Ş. – AAC block and AAC Blocks for Floor Plates
Publisher
Institut Bauen und Umwelt e.V. Tel +49 (0)30 3087748- 0
Panoramastr. 1 Fax +49 (0)30 3087748- 29
10178 Berlin Mail info@ibu-epd.com
Germany Web www.ibu-epd.com
Programme holder
Institut Bauen und Umwelt e.V. Tel +49 (0)30 - 3087748- 0
Panoramastr 1 Fax +49 (0)30 – 3087748 - 29
10178 Berlin Mail info@ibu-epd.com
Germany Web www.ibu-epd.com
Author of the Life Cycle
Assessment Tel +90 216 410 61 35
Altensis Ins. Enerji San. Ve Tic. Ltd. Fax +90 216 410 61 53
Sti. Mail info@altensis.com
Kayisdagi Caddesi Baris Sok. Meriç Web www.altensis.com
Plaza 2
34750 Istanbul
Turkey
Owner of the Declaration
Türk Ytong A.S. Tel + 90 216 396 66 00
Aydinevler Mahallesi, Inönü Caddesi, Fax + 90 216 396 19 61
Gökçe Sokak, Maltepe No:3 Mail ytong@ytong.com.tr
34854 Istanbul Web www.ytong.com.tr
Turkey
