ver1 2015
ENVIRONMENTAL PRODUCT DECLARATION
in accordance with ISO 14025, ISO 21930 and EN 15804
Owner of the declaration: Skanska Industrial Solutions AB
Program operator: The Norwegian EPD Foundation
Publisher: The Norwegian EPD Foundation
Declaration number: NEPD-2514-1242-EN
Registration number: NEPD-2514-1242-EN
ECO Platform reference number: -
Issue date: 10.11.2020
Valid to: 10.11.2025
ABT 16 Vällsta Asphalt Plant
Skanska Industrial Solutions AB
www.epd-norge.no
NEPD-2514-1242-EN ABT 16 Vällsta Asphalt Plant 1 / 8
General information
Product: Owner of the declaration:
ABT 16 Vällsta Asphalt Plant Skanska Industrial Solutions AB
Contact person: Henrik Sjöholm
Phone: +46 10-448 71 06
e-mail: Henrik.Sjoholm@Skanska.se
Program operator: Manufacturer:
The Norwegian EPD Foundation Skanska Industrial Solutions AB
Pb. 5250 Majorstuen, 0303 Oslo
Phone: +47 23 08 80 00
e-mail: post@epd-norge.no
Declaration number: Place of production:
Vällsta Asfaltverk
NEPD-2514-1242-EN Rydholmsvägen 7
19491 Upplands Väsby
ECO Platform reference number: Management system:
ISO 14001, ISO 9001
This declaration is based on Product Category Rules: Organisation no:
556793-1638
CEN Standard EN 15804:2012+A1:2013 serves as core PCR
NPCR 025:2017 Part B for Asphalt
Statement of liability: Issue date: 10.11.2020
The owner of the declaration shall be liable for the underlying information and
evidence. EPD Norway shall not be liable with respect to manufacturer Valid to: 10.11.2025
information, life cycle assessment data and evidences.
Declared unit: Year of study:
1 tonne ABT 16 Vällsta Asphalt Plant 2019
Declared unit with option: Comparability:
EPD of construction products may not be comparable if they not comply with EN
A1,A2,A3,A4
15804 and seen in a building context.
Functional unit: Author of the Life Cycle Assessment:
The declaration is developed using eEPD v4.0 from LCA.no
Approval:
Company specific data are:
Collected/registered by: Henrik Sjoholm
Internal verification by: Nicklas Magnusson
Verification: Approved:
Independent verification of data, other environmental information and the
declaration according to ISO14025:2010, § 8.1.3 and § 8.1.4
External
Third party verifier:
Sign Sign
Martin Erlandsson, IVL Swedish Environmental Research Institute
(Independent verifier approved by EPD Norway)
NEPD-2514-1242-EN ABT 16 Vällsta Asphalt Plant 2 / 8
Product
Product description: Technical data:
Asphalt Wearing course for road contruction.
ABT 16 wearing course according to Swedish road administration specification
Product specification TDOK 2013:0529.
ABT 16 (AC 16) Market:
Materials % Sweden
Aggregate 56,10
Reference service life, product
Bitumen 3,90
Amin, CAS Nr. 68910-93-0 0,01 Depending on traffic, road design and climate conditions.
Bitumen from reclaimed asphalt 2,00 Reference service life, construction works
Aggregates from reclaimed asphalt 38,00
Depending on traffic, road design and climate conditions.
LCA: Calculation rules
Declared unit: Allocation:
The allocation is made in accordance with the provisions of EN 15804.
1 tonne ABT 16 Vällsta Asphalt Plant
Incoming energy and water and waste production in-house is allocated
Cut-off criteria: equally among all products through mass allocation. Effects of primary
production of recycled materials is allocated to the main product in which the
All major raw materials and all the essential energy is included. The
material was used. The recycling process and transportation of the material is
production processes for raw materials and energy flows with very small
allocated to the analysis in this EPD. For bitumen production, crude oil
amounts (less than 1%) are not included. These cut-off criteria do not
extraction and transport are allocated by mass, while the final products from oil
apply for hazardous materials and substances.
refineries are allocated by economic factors.
Data quality:
Specific data for the product composition are provided by the manufacturer. They represent the production of the declared product and were collected for EPD
development in the year of study. Background data is based on registered EPDs according to EN 15804, Ostfold Research databases, ecoinvent and other LCA
databases. The data quality of the raw materials in A1 is presented in the table below.
Specific environmental data from EPDs (Skanska EPD), in accordance with EN 15804, have been used for aggregates. Similarly, specific data have been used for
transport distances from supplier to asphalt plant and for all factory data (energy use, waste quantities, etc.). For all other data, generic data available in EPD tool
v4.0 have been used. Transport of reclaimed asphelt from the road to asphalt factory includes a return distance.
For bitumen, generic data from Eurobitume is used because specific data cannot be determined from the mix of bitumen suppliers according to EU standards
etc. used by Skanska.
Environmental impact for reclaimed asphalt falls to previous product systems until arrival at the asphalt plant. The asphalt plant uses electricity marked "Good
Environmental Choice".
Materials Source Data quality Year
Bitumen Eurobitume Database 2012
Aggregate NEPD-1257-403 EPD 2016
Aggregates from reclaimed asphalt Østfoldforskning Database 2017
Bitumen from reclaimed asphalt Østfoldforskning Database 2017
Amin, CAS Nr. 68910-93-0 Supplier Eco footprint 2020
NEPD-2514-1242-EN ABT 16 Vällsta Asphalt Plant 3 / 8
System boundary:
Additional technical information:
40% reclaimed asphalt is included.
40% renewable energy used in production (A3).
NEPD-2514-1242-EN ABT 16 Vällsta Asphalt Plant 4 / 8
LCA: Scenarios and additional technical information
The following information describe the scenarios in the different modules of the EPD.
Transport from production place to user (A4)
Capacity utilisation Fuel/Energy
Type Type of vehicle Distance km Unit Value (l/t)
(incl. return) % consumption
Truck 50,0 % Asfaltbil med henger, EURO 6 50 0,023668 l/tkm 1,18
Railway l/tkm
Boat l/tkm
Other Transportation l/tkm
NEPD-2514-1242-EN ABT 16 Vällsta Asphalt Plant 5 / 8
LCA: Results
The LCA results are presented below for the declared unit defined on page 2 of the document.
System boundaries (X=included, MND=module not declared, MNR=module not relevant)
Construction Beyond the
Product stage installation User stage End of life stage . system
stage bondaries
A1 A2 A3 A4 A5 B1 B2 B3 B4 B5 B6 B7 C1 C2 C3 C4 . D
X X X X MND MND MND MND MND MND MND MND MND MND MND MND . MND
Environmental impact
Parameter Unit A1-A3 A4
GWP* kg CO 2 -eq 3,19E+01 4,34E+00
ODP kg CFC11 -eq 3,80E-06 9,00E-07
POCP kg C 2H 4-eq 1,46E-02 6,83E-04
AP kg SO 2 -eq 1,97E-01 1,13E-02
EP kg PO 3- -eq 3,89E-02 1,55E-03
4
ADPM kg Sb -eq 2,26E-05 1,08E-05
ADPE MJ 2,05E+03 7,13E+01
GWP Global warming potential; ODP Depletion potential of the stratospheric ozone layer; POCP Formation potential of tropospheric photochemical oxidants;
AP Acidification potential of land and water; EP Eutrophication potential; ADPM Abiotic depletion potential for non fossil resources; ADPE Abiotic depletion
potential for fossil resources
"Reading example: 9,0 E-03 = 9,0*10-3 = 0,009"
*INA Indicator Not Assessed
*Remarks to environmental impacts
The results for GWP exclude biogenic CO2 (IPCC 2007)
waR slairetam tropsnarT gnirutcafunaM tropsnarT ylbmessA esU ecnanetniaM riapeR tnemecalpeR tnemhsibrufeR lanoitarepO ygrene esu lanoitarepO esu
retaw
-eD noitcurtsnoc noitilomed tropsnarT etsaW gnissecorp lasopsiD -yrevoceR-esueR -gnilcyceR laitnetop
NEPD-2514-1242-EN ABT 16 Vällsta Asphalt Plant 6 / 8
Resource use
Parameter Unit A1-A3 A4
RPEE MJ 1,75E+02 1,30E+00
RPEM MJ 1,07E+00 0,00E+00
TPE MJ 1,76E+02 1,30E+00
NRPE MJ 4,05E+02 7,35E+01
NRPM MJ 2,60E+03 0,00E+00
TRPE MJ 2,12E+03 7,35E+01
SM kg 4,00E+02 0,00E+00
RSF MJ 2,82E-02 0,00E+00
NRSF MJ 0,00E+00 0,00E+00
W m3 4,77E+00 1,74E-02
RPEE Renewable primary energy resources used as energy carrier; RPEM Renewable primary energy resources used as raw materials; TPE Total use of renewable
primary energy resources; NRPE Non renewable primary energy resources used as energy carrier; NRPM Non renewable primary energy resources used as
materials; TRPE Total use of non renewable primary energy resources; SM Use of secondary materials; RSF Use of renewable secondary fuels; NRSF Use of non
renewable secondary fuels; W Use of net fresh water
"Reading example: 9,0 E-03 = 9,0*10-3 = 0,009"
*INA Indicator Not Assessed
End of life - Waste
Parameter Unit A1-A3 A4
HW kg 2,38E-03 3,97E-05
NHW kg 4,09E+00 6,71E+00
RW kg INA* INA*
HW Hazardous waste disposed; NHW Non hazardous waste disposed; RW Radioactive waste disposed
"Reading example: 9,0 E-03 = 9,0*10-3 = 0,009"
*INA Indicator Not Assessed
End of life - Output flow
Parameter Unit A1-A3 A4
CR kg 0,00E+00 0,00E+00
MR kg 5,20E-02 0,00E+00
MER kg 0,00E+00 0,00E+00
EEE MJ INA* INA*
ETE MJ INA* INA*
CR Components for reuse; MR Materials for recycling; MER Materials for energy recovery; EEE Exported electric energy; ETE Exported thermal energy
"Reading example: 9,0 E-03 = 9,0*10-3 = 0,009"
*INA Indicator Not Assessed
NEPD-2514-1242-EN ABT 16 Vällsta Asphalt Plant 7 / 8
Additional Norwegian requirements
Greenhouse gas emissions from the use of electricity in the manufacturing phase
National production mix from import, low voltage (production of transmission lines, in addition to direct emissions and losses in grid) of applied electricity for the
manufacturing process (A3).
Electricity mix Data source Amount Unit
El-mix, Sweden (kWh) ecoinvent 3.4 Alloc Rec 42,67 g CO2-ekv/kWh
Dangerous substances
The product contains no substances given by the REACH Candidate list or the Norwegian priority list.
Indoor environment
Bibliography
ISO 14025:2010 Environmental labels and declarations - Type III environmental declarations - Principles and procedures.
ISO 14044:2006 Environmental management - Life cycle assessment - Requirements and guidelines.
EN 15804:2012+A1:2013 Environmental product declaration - Core rules for the product category of construction products.
ISO 21930:2017 Sustainability in buildings and civil engineering works, Core rules for environmental product declarations of construction products.
ecoinvent v3, Alloc Rec, Swiss Centre of Life Cycle Inventories.
Iversen et al., (2018) eEPD v3.0 – Background information for EPD generator system, LCA.no report number 04.18.
Iversen et al., (2017) EPD generator for Asfalt, Bakgrunnsrapport for applikasjon og datagrunnlag, OR 11.17, Østfoldforskning.
NPCR Part A: Construction products and services. Ver. 1.0. April 2017, EPD-Norge.
NPCR Part B for Asphalt. NPCR 025 Ver. 1.1. December 2017, EPD-Norge.
Inventory report, LCA- inventeringsrapport EPD asfalt ABT 16 Vällsta 2020.
Program operator and publisher Phone: +47 23 08 80 00
The Norwegian EPD Foundation
Post Box 5250 Majorstuen, 0303 Oslo e-mail: post@epd-norge.no
0303 Oslo Norway web: www.epd-norge.no
Owner of the declaration Phone: +46 10-448 71 06
Skanska Industrial Solutions AB Fax:
Warfvinges väg 25 e-mail: Henrik.Sjoholm@Skanska.se
112 74 Stockholm web: www.skanska.se
Author of the Life Cycle Assessment Phone: +47 69 35 11 00
Østfoldforskning AS Fax: +47 69 34 24 94
Stadion 4 e-mail:
1671 Kråkerøy web: www.ostfoldforskning.no
Developer of EPD generator Phone: +47 916 50 916
LCA.no AS
Dokka 1C e-mail: post@lca.no
1671 Kråkerøy web: www.lca.no
NEPD-2514-1242-EN ABT 16 Vällsta Asphalt Plant 8 / 8
