ENVIRONMENTAL-PRODUCT DECLARATION
as per ISO 14025 and EN 15804+A2
Owner of the Declaration ACO Ahlmann SE & Co. KG
Publisher Institut Bauen und Umwelt e.V. (IBU)
Programme holder Institut Bauen und Umwelt e.V. (IBU)
Declaration number EPD-ACO-20220221-IBA2-EN
Issue date 22/12/2022
Valid to 21/12/2027
ACO gravel grid eco
ACO Ahlmann SE & Co. KG
www.ibu-epd.com | https://epd-online.com
1. General Information
ACO Ahlmann SE & Co. KG ACO gravel grid eco
Programme holder Owner of the declaration
IBU – Institut Bauen und Umwelt e.V. ACO Ahlmann SE & Co. KG
Hegelplatz 1 Am Ahlmannkai -
10117 Berlin 24782 Büdelsdorf
Germany Germany
Declaration number Declared product / declared unit
EPD-ACO-20220221-IBA2-EN 1m² of the product ACO gravel grid eco, without filling material
This declaration is based on the product category rules: Scope:
Permanent way materials for outdoor traffic routes, 01/08/2021 This EPD refers to 1 m² of the ACO gravel grid eco and is valid for four
(PCR checked and approved by the SVR) product variants (eco grey, eco black, eco S and eco M, without filling
material). The product is manufactured in Büdelsdorf, Germany. The Life
Cycle Assessment is based on data covering the reference year 2022
Issue date (from January to May).
The owner of the declaration shall be liable for the underlying information
22/12/2022
and evidence; the IBU shall not be liable with respect to manufacturer
information, life cycle assessment data and evidences.
Valid to
The EPD was created according to the specifications of EN 15804+A2. In
21/12/2027 the following, the standard will be simplified as EN 15804 bezeichnet.
Verification
The standard EN 15804 serves as the core PCR
Independent verification of the declaration and data according to ISO
14025:2011
internally X externally
Dipl.-Ing Hans Peters
(chairman of Institut Bauen und Umwelt e.V.)
Florian Pronold Prof. Dr. Birgit Grahl,
(Managing Director Institut Bauen und Umwelt e.V.) (Independent verifier)
1 Environmental-Product Declaration - ACO Ahlmann SE & Co. KG - ACO gravel grid eco
2. Product
Name Value Unit
2.1 Product description/Product definition
Gross density acc. DIN EN ISO 845 910 kg/m3
The ACO gravel grid eco (ACO Kiesstabilisierung eco grey and
black article no. 281095 and 281092, ACO Self® Kieswabe eco Deviation of the dimensions (acceptable), acc. 3 mm
S and M article no. 281090 and 281091) is used for the DIN 16742 TG5
simultaneous unsealing and stabilisation of gravel surfaces. Permissible difference of the two diagonals
The ACO gravel grid eco is an ecological outdoor reinforcement (only for rectangular blocks with sizes of over 5 mm
system that on the one hand, is used to stabilise gravel and 300 mm.), acc. DIN 16742 TG5
chippings in an environmentally friendly and visually appealing Pressure stable, acc. DIN EN 1991-1-1 300 t/m²
way and, on the other hand, allows rainwater to seep away
Tensile elastic modulus, acc. DIN EN ISO 527-
naturally directly onto the surface of the property. 1100 MPa
1
Properly laid, a barrier-free, stable and 100% water-permeable
UV-
surface is created, that can be walked on and driven over. This UV-stable -
stable
prevents ponding. The honeycomb structure of the mats holds
Live load (axle load 2.2 t and max. total weight
the gravel securely in place when, for example, pedestrians, approved -
3.5 t)
cyclists or cars move over the surface. Wheel tracks of any kind
are avoided and less gravel is needed compared to loose Performance data of the product with respect to its
stones. An individual design is possible with fine chippings or characteristics in accordance with the relevant technical
decorative gravel. provision (no CE-marking).
The integrated 100% water-permeable geotextile
(polypropylene) is untearable connected to the grid. This means 2.4 Delivery status
that the gravel cannot undermine the product and stays in The dimensions (l x w x h) of the ACO gravel grid eco are as
place. Furthermore, weeds cannot root through the geotextile. follows:
The overlap of the geotextile is optimised for laying the ACO
gravel grid eco. eco grey and black 120 x 160 x 3 cm
The honeycombs are made of 100% recycled polypropylene
(post-consumer recycled plastic) and the entire product was eco M: 120
awarded the "Blue Angel" in 2021. x 80 x 3 cm
Using a patented injection moulding process, the ACO gravel
grid eco is produced by ACO in Germany. eco S: 80
x 60 x 3 cm
For the use and application of the product, the respective
national provisions at the place of use apply, in Germany for The products are delivered on euro-palettes with total weight
example the building codes of the federal states and the per pallet of approx. 70 kg and dimensions
corresponding national specifications. [Alternative 3: Product 120 x 80 x 117 cm (l x w x h).
for which no legal provisions for harmonisation of the EU exist]:
For the use and application of the product the respective 2.5 Base materials/Ancillary materials
national provisions at the place of use apply, in Germany for The ACO gravel grid eco is made completely of polypropylene
example the building codes of the federal states and the with 96 M.-% post-consumer recycling polypropylene for the
corresponding national specifications. honeycombs and 4 M.-% primary polypropylene for the
geotextile.
2.2 Application This product/article/at least one partial article contains
The ACO gravel grid eco can be used in a variety of ways in the substances listed in the candidate list (date: 10.06.2022)
design of unsealed outdoor areas with a slope of up to 10%, exceeding 0.1 percentage by mass: no
such as garden paths and terraces, municipal landscaping (e.
g. parks, cemeteries), seating areas, courtyard areas, parking This product/article/at least one partial article contains other
spaces, access roads and driveways. carcinogenic, mutagenic, reprotoxic (CMR) substances in
The ACO gravel grid is both walkable and in its installed state categories 1A or 1B which are not on the candidate list,
drivable by bicycle, wheelchair, motorbike and car with a load of exceeding 0.1 percentage by mass: no
up to 300 t/m² (according to DIN EN 1991-1-1). ACO gravel grid
eco is approved for vehicles with an axle load of 2.2 t and a Biocide products were added to this construction product or it
max. total weight of 3.5 t. has been treated with biocide products (this then concerns a
treated product as defined by the (EU) Ordinance on Biocide
2.3 Technical Data
Products No. 528/2012): no
The technical specifications of the products within the scope of
the EPD shall be listed, including the reference to the test 2.6 Manufacture
methods/test standards for each specification. The ACO gravel grid eco is produced using an injection
moulding process at the production site in Germany,
For products with CE marking, the technical specifications must Büdelsdorf. The polypropylene granules are melted in an
be specified in accordance with information in the declaration of extruder and the product is formed by injection moulding.
performance. The properties relevant to the product should be During injection moulding, the product is actively cooled. After
specified in the table below. If no information is given for forming the product is passively cooled. The product is then
properties, an explanation must be given in the background demoulded and palletised.
report to the EPD as to why the property is not relevant to the The ACO Ahlmann SE & Co. KG production site is certified
product. according to the ISO 9001 quality management system.
2.7 Environment and health during manufacturing
Constructional data
2 Environmental-Product Declaration - ACO Ahlmann SE & Co. KG - ACO gravel grid eco
During the manufacturing process, no environmentally Erhaltung und Modernisierung von Bauwerken e. V. (IEMB
hazardous or harmful emissions are produced. The product is 2008)", the reference service life corresponds to 20 years.
made completely of polypropylene and there are no mixtures of Description of the influences on the ageing of the product when
materials. The production losses are fully recycled. applied in accordance with the rules of technology.
The ACO Ahlmann SE & Co. KG production site is certified
2.13 Extraordinary effects
according to the ISO 50001 energy management system and
ISO 14001 environmental management system. Fire
Information on the fire performance is not relevant as the
2.8 Product processing/Installation product is only used outdoors.
The subfloor profile must be determined according to local Water
conditions and with a view to suitability for the anticipated load. ACO gravel grids support natural water circulation as the
For detailed processing steps regarding the different declared products are 100% water-permeable. Furthermore, it
applications (walkable and drivable), please refer to the contributes to the reduction of water-impermeable surfaces and
installation instructions. thus to the reduction of flooding.
Generally, a levelled sand layer over a crushed stone layer is The materials of the declared products are selected in such a
required. For the use of footpaths and cycle paths, the gravel way that, when properly installed, they do not release water-
layer may be omitted. In any case, the soil structure must be soluble substances into the environment that could lead to the
mechanically compacted (e. g. vibrating plate compactor). contamination of water bodies according to DIN EN ISO 71-3
and DIN EN 62321-3-1.
The mats are laid staggered on the compacted sand layer. It is
advantageous to lay the mats in a bond, preferably across the Mechanical destruction
direction of travel. The ACO gravel grid eco can be laid on If installed and used properly, the top layer of 1.5 to
surfaces with a slope of up to 10%. From a slope of 5%, 2 cm protects the ACO gravel grid eco mats. In the event of
additional ground nails must be used. The ACO gravel grid eco unforeseen mechanical destruction, the ACO gravel grid eco
is then filled with gravel and compacted. can be replaced and recycled.
2.14 Re-use phase
For maximum longevity the ACO gravel grid eco should always
be completely covered with a gravel layer of approx. 1.5 to 2 Sustainable recycling is possible with the ACO gravel grid eco.
cm. It is made completely of polypropylene, which consequently
does not require a hazardous waste disposal. The mats can be
2.9 Packaging added back to the recycling system without prior separation.
The ACO gravel grid eco is palletised on a euro-pallet and The top layer protects the product from environmental
wrapped with polyethylene foil. The edges are secured with influences, so that reuse is conceivable.
cardboard.
2.15 Disposal
2.10 Condition of use The waste key codes in accordance with the European Waste
No unusual material changes in the state of installation are Catalogue (EWC) are listed below.
known for the materials used in the ACO gravel grid eco. The Product waste
used materials polypropylene and recycled polypropylene are EWC 17 02 03 Plastic
UV-stabilised and weather-resistant. The ACO gravel grid eco is
resistant to engine oils and fuels, for example. Packaging waste
EWC 15 01 02 Plastic packaging
2.11 Environment and health during use EWC 15 01 03 Wooden packaging
There are no known negative interactions between the ACO
gravel grid, the environment and health. ACO gravel grids help 2.16 Further information
to create unsealed drivable surfaces and support the natural Further information about the company, products and contact
water cycle. details can be found on the following websites:
The ACO gravel grid eco is a 100% water-permeable product. English
The infiltration capacity depends on the condition of the soil and https://www.aco.com/en/
not on the product. https://www.buildingmaterial.aco
2.12 Reference service life German
The ACO gravel grid eco is a long-lasting product. The https://www.aco-hochbau.de
polypropylene materials used have a service life of 100 years. https://www.aco.shop/de/de/hochbau
Due to the stresses in the installed state and based on the
service life data of selected components from the "Institut für
3. LCA: Calculation rules
values must be made, e.g. concerning variability of the
3.1 Declared Unit production process, geographical representativeness and the
The declared unit is 1 m², with 1.44 kg/m². influence of background data and preliminary products
Declared unit compared to the environmental impacts caused by actual
production.
Name Value Unit
Declared unit 1 m2
Grammage 1.44 kg/m2 3.2 System boundary
The type of the EPD is "cradle-to-gate" with options. The
For IBU core EPDs (where clause 3.6 is part of the EPD): for
modules considered in the Life Cycle Assessment are modules
average EPDs, an estimate of the robustness of the LCA
A1-A3, A4, A5, C and D. The declaration for Module B was
3 Environmental-Product Declaration - ACO Ahlmann SE & Co. KG - ACO gravel grid eco
excluded as the product does not cause any environmental polypropylene are declared.
impacts during its service life. Module D/2
This module includes potential benefits from energy recovery of
Modules A1-A3 the incineration of the product.
The product stage involves raw material supply, the transport of
the raw materials and the manufacturing process of injection 3.3 Estimates and assumptions
moulding, including all energy and water consumption during The recycling polypropylene is declared as secondary material
manufacturing. The production of the packaging is also and modelled as a burden-free input. Therefore, no benefits are
included in module A3. declared in module D/1 for recycling.
3.4 Cut-off criteria
For the environmental impact, the use of green
electricity was calculated. The proportion of the electricity A slip additive with 0.5 M.-% and UV stabilizers with 0.2 M.-%
demand covered by were not included in the Life Cycle Assessment. The safety
green electricity in the total electricity demand is 100%. data sheets of the slip additive and UV stabilizers show that
there is no environmental hazard.
Module A4
3.5 Background data
This module considers the environmental impact of transport
The model of the ACO gravel grid eco was made using the
from the production site to the construction site.
GaBi ts software. For the background data of the Life Cycle
Assessment the database ecoinvent 3
Module A5
(version 3.6) was used.
The installation is indicated without the filling material and sand
or gravel for the underground preparation, as different 3.6 Data quality
quantities are required for the installation depending on the
The data was compiled product-specifically and under
subgrade and the application of the load class.
consistent methodical and boundary conditions.
The environmental impacts of the incineration of plastic,
The data quality for the foreground data can be described as
cardboard and wood packaging are indicated.
good, and the data quality for the background data can be
described as mean because some data sets are older than 10
Module C1
years.
The deconstruction of the product is done manually, therefore
no energy is needed. 3.7 Period under review
The foreground data refers to the manufacturing process for the
Module C2 year 2022 (January to May). The data refers to an average of
This module includes the transport to waste treatment. this time period and can be transferred as an average value to
a whole year.
Module C3
This module includes the environmental impacts of waste 3.8 Geographic Representativeness
treatment of the product at the end of life. Two scenarios were Land or region, in which the declared product system is
declared. manufactured, used or handled at the end of the product´s
Module C3/1 lifespan: Europe
100% recycling of the product.
Module C3/2
100% incineration of the product and energy recovery. 3.9 Allocation
During the manufacturing process, no co-products are
Module C4 generated. Input and output flows are all allocated to the
No landfilling scenario is considered for the Life Cycle calculated product system. No allocation in the foreground data
Assessment, so this module is declared zero. for the considered product system is necessary.
Information about allocations of the background data can be
Module D found in the documentation of the data sets for the ecoinvent 3
According to module C3, two scenarios for module D are database.
declared.
3.10 Comparability
The potential benefits for energy recovery from the incineration
of packaging material in module A5 are declared in both Basically, a comparison or an evaluation of EPD data is only
scenarios. possible if all the data sets to be compared were created
according to EN 15804 and the building context, respectively
Module D/1 the product-specific characteristics of performance, are taken
This module includes potential benefits for the recycling of into account.
primary polypropylene, but no benefits for recycled The used background database has to be mentioned.
4. LCA: Scenarios and additional technical information
Characteristic product properties
Information on describing the biogenic Carbon Content at
Information on biogenic carbon
factory gate
Name ValueUnit
The product does not contain biogenic carbon. The packaging
(euro-pallet and cardboard) contains 0.09 kg biogenic carbon kg
Biogenic carbon content in product -
for the declared unit of 1 m² ACO gravel grid eco. In module A5 C
the biogenic carbon of the packaging leaves the product Biogenic carbon content in accompanying kg
0.09
system. packaging C
4 Environmental-Product Declaration - ACO Ahlmann SE & Co. KG - ACO gravel grid eco
addition, it shall be stated that the RSL applies for the reference
The following technical information is a basis for the declared conditions only.
modules.
The same holds for a service life declared by the manufacturer.
Transport from the gate to the site (A4)
Corresponding information related to in-use conditions needs
Name Value Unit
not be provided if a service life taken from the list on service life
Transport distance 100 km by BNB is declared.
Capacity utilisation (including empty runs) 67 %
End of life (C1-C4)
Assembly (A5)
Name Value Unit
Name Value Unit
Collected separately waste type waste type 1.44 kg
PE foil (*46 MJ/kg) 0.009 kg
Recycling (C3/1) 1.44 kg
Cardboard (*18 MJ/kg) 0.1 kg
Energy recovery (C3/2) 1.44 kg
Euro-pallet (*18 MJ/kg) 0.1 kg
Waste for disposal C4 0 kg
*Heating value
Transport distance 50 km
Capacity utilisation (including empty runs) 67 %
Reference service life
Name ValueUnit
Reuse, recovery and/or recycling potentials (D), relevant
Reference service life (according to IEMB, see § 20 a scenario information
2.12) In D/1 the potential benefit of the recycling of the primary
polypropylene (geotextile) and the incineration of the packaging
In case a reference service life according to applicable ISO is declared. In module D/2 the potential benefit of the energy
standards is declared then the assumptions and in-use recovery for the incineration of the product and the packaging is
conditions underlying the determined RSL shall be declared. In declared.
5 Environmental-Product Declaration - ACO Ahlmann SE & Co. KG - ACO gravel grid eco
5. LCA: Results
In the table "Description of the system boundary", all declared modules are indicated with an "X". As default the modules B3, B4, B5
are marked as "MNR" module not relevant. Module B is not relevant for the product system, so modules B1, B2, B6 and B7 are marked
as "ND" not declared. The categories of waste disposed are marked as "ND", because the waste categories cannot be declared from
the datasets of the ecoinvent 3.6 database.
DESCRIPTION OF THE SYSTEM BOUNDARY (X = INCLUDED IN LCA; ND = MODULE OR INDICATOR NOT DECLARED; MNR =
MODULE NOT RELEVANT)
BENEFITS
AND LOADS
CONSTRUCTION
BEYOND
PRODUCT STAGE PROCESS USE STAGE END OF LIFE STAGE
THE SYSTEM
STAGE
BOUNDARIE
S
la ire ta m w a Ry lp p u s tro p s n a rT g n iru tc a fu n a M e h t m o rf tro p s n a rTe tis e h t o t e ta g y lb m e s s A e s U e c n a n e tn ia M ria p e R tn e m e c a lp e R tn e m h s ib ru fe R y g re n e la n o ita re p Oe s u re ta w la n o ita re p Oe s u n o itc u rts n o c -e Dn o itilo m e d tro p s n a rT g n is s e c o rp e ts a W la s o p s iD -e s u e R-y re v o c e R-g n ilc y c e Rla itn e to p
A1 A2 A3 A4 A5 B1 B2 B3 B4 B5 B6 B7 C1 C2 C3 C4 D
X X X X X MND MND MNR MNR MNR MND MND X X X X X
RESULTS OF THE LCA - ENVIRONMENTAL IMPACT according to EN 15804+A2: 1 m² ACO gravel grid eco
Parameter Unit A1-A3 A4 A5 C1 C2 C3/1 C3/2 C4 D/1 D/2
GWP-total kg CO 2 eq 2.48E-01 2.28E-02 3.19E-01 0 9.38E-03 5.3E-01 3.43E+00 0 -1.71E-01 -1.16E-01
GWP-fossil kg CO 2 eq 5.44E-01 2.27E-02 2.6E-02 0 9.37E-03 5.32E-01 3.43E+00 0 -1.69E-01 -1.14E-01
GWP-
biogenic kg CO 2 eq -2.96E-01 1.72E-05 2.93E-01 0 7.1E-06 -2.22E-03 2.41E-04 0 -1.79E-03 -2.03E-03
GWP-luluc kg CO 2 eq 5.55E-04 7.22E-06 6.23E-07 0 2.97E-06 3.12E-04 2.06E-05 0 -1.31E-04 -1.59E-04
ODP kg CFC11 eq 6.62E-08 5.59E-09 2.6E-10 0 2.3E-09 3.87E-08 8.14E-09 0 -9.22E-09 -1.14E-08
AP mol H+ eq 2.46E-03 7.32E-05 3.6E-05 0 3.01E-05 1.53E-03 7.91E-04 0 -6.26E-04 -4.56E-04
EP-
kg P eq 1.4E-04 1.68E-06 1.38E-06 0 6.92E-07 7.99E-05 9.76E-06 0 -5.85E-05 -6.8E-05
freshwater
EP-marine kg N eq 5.2E-04 1.64E-05 1.87E-05 0 6.75E-06 5.81E-04 4.45E-04 0 -1.1E-04 -8.04E-05
EP-terrestrial mol N eq 5.27E-03 1.79E-04 1.81E-04 0 7.37E-05 4.61E-03 3.79E-03 0 -1.12E-03 -7.84E-04
kg NMVOC
POCP 1.83E-03 7.03E-05 4.44E-05 0 2.89E-05 1.5E-03 9.19E-04 0 -4.28E-04 -2.18E-04
eq
ADPE kg Sb eq 7.19E-06 4.05E-07 4.22E-08 0 1.67E-07 6.55E-06 1.14E-06 0 -1.13E-06 -5.11E-07
ADPF MJ 1.14E+01 3.71E-01 3.04E-02 0 1.53E-01 5.51E+00 6.7E-01 0 -4.91E+00 -2.32E+00
m3 world eq
WDP 2.84E-01 1.81E-03 -1.74E-03 0 7.44E-04 1.21E-01 2.18E-01 0 -7.61E-02 -5.19E-02
deprived
GWP = Global warming potential; ODP = Depletion potential of the stratospheric ozone layer; AP = Acidification potential of land and water; EP =
Eutrophication potential; POCP = Formation potential of tropospheric ozone photochemical oxidants; ADPE = Abiotic depletion potential for non-fossil
resources; ADPF = Abiotic depletion potential for fossil resources; WDP = Water (user) deprivation potential)
RESULTS OF THE LCA - INDICATORS TO DESCRIBE RESOURCE USE according to EN 15804+A2: 1 m² ACO gravel grid eco
Parameter Unit A1-A3 A4 A5 C1 C2 C3/1 C3/2 C4 D/1 D/2
PERE MJ 4.9E+00 4.65E-03 4.86E+00 0 1.92E-03 2.58E-01 2.37E-02 0 -2.25E-01 -2.63E-01
PERM MJ 3.24E+00 0 -3.24E+00 0 0 0 0 0 0 0
PERT MJ 9.76E+00 4.65E-03 6.36E-04 0 1.92E-03 2.58E-01 2.37E-02 0 -2.25E-01 -2.63E-01
PENRE MJ 8.63E+00 3.71E-01 4.44E-01 0 1.53E-01 7.68E+00 3.02E+00 0 -4.91E+00 -2.32E+00
PENRM MJ 2.76E+00 0 -4.14E-01 0 0 -2.35E+00 -2.35E+00 0 0 0
PENRT MJ 1.14E+01 3.71E-01 3.04E-02 0 1.53E-01 5.51E+00 6.7E-01 0 -4.91E+00 -2.32E+00
SM kg 1.41E+00 0 0 0 0 0 0 0 5.16E-02 0
RSF MJ 0 0 0 0 0 0 0 0 0 0
NRSF MJ 0 0 0 0 0 0 0 0 0 0
FW m3 6.61E-03 4.2E-05 -4.05E-05 0 1.73E-05 2.83E-03 5.07E-03 0 -1.77E-03 -1.21E-03
PERE = Use of renewable primary energy excluding renewable primary energy resources used as raw materials; PERM = Use of renewable primary
energy resources used as raw materials; PERT = Total use of renewable primary energy resources; PENRE = Use of non-renewable primary energy
excluding non-renewable primary energy resources used as raw materials; PENRM = Use of non-renewable primary energy resources used as raw
materials; PENRT = Total use of non-renewable primary energy resources; SM = Use of secondary material; RSF = Use of renewable secondary fuels;
NRSF = Use of non-renewable secondary fuels; FW = Use of net fresh water
RESULTS OF THE LCA – WASTE CATEGORIES AND OUTPUT FLOWS according to EN 15804+A2:
1 m² ACO gravel grid eco
Parameter Unit A1-A3 A4 A5 C1 C2 C3/1 C3/2 C4 D/1 D/2
HWD kg ND ND ND ND ND ND ND ND ND ND
NHWD kg ND ND ND ND ND ND ND ND ND ND
6 Environmental-Product Declaration - ACO Ahlmann SE & Co. KG - ACO gravel grid eco
RWD kg ND ND ND ND ND ND ND ND ND ND
CRU kg 0 0 0 0 0 0 0 0 0 0
MFR kg 1.61E-02 0 0 0 0 1.44E+00 0 0 0 0
MER kg 0 0 0 0 0 0 0 0 0 0
EEE MJ 0 0 3.48E-01 0 0 0 1.8E-01 0 0 0
EET MJ 0 0 6.97E-01 0 0 0 3.52E-01 0 0 0
HWD = Hazardous waste disposed; NHWD = Non-hazardous waste disposed; RWD = Radioactive waste disposed; CRU = Components for re-use;
MFR = Materials for recycling; MER = Materials for energy recovery; EEE = Exported electrical energy; EET = Exported thermal energy
RESULTS OF THE LCA – additional impact categories according to EN 15804+A2-optional:
1 m² ACO gravel grid eco
Parameter Unit A1-A3 A4 A5 C1 C2 C3/1 C3/2 C4 D/1 D/2
Disease
PM 3.48E-08 2E-09 3.58E-10 0 8.22E-10 2.65E-08 3.74E-09 0 -3.66E-09 -1.33E-09
incidence
IR kBq U235 eq 5.58E-02 1.88E-03 6.9E-05 0 7.75E-04 2.87E-02 2.08E-03 0 -2.98E-02 -3.68E-02
ETP-fw CTUe 1.13E+01 3.07E-01 5.59E-02 0 1.26E-01 6.09E+00 7.2E+00 0 -1.34E+00 -1.25E+00
HTP-c CTUh 2.81E-10 7.14E-12 8.99E-12 0 2.94E-12 5.64E-10 2.99E-10 0 -3.91E-11 -3.06E-11
HTP-nc CTUh 6.61E-09 2.8E-10 4.58E-10 0 1.15E-10 7.67E-09 1.18E-08 0 -1.26E-09 -1.05E-09
SQP SQP 3.82E+01 4.22E-01 9.34E-03 0 1.74E-01 4.22E+00 2.06E-01 0 -3.46E-01 -3.74E-01
PM = Potential incidence of disease due to PM emissions; IR = Potential Human exposure efficiency relative to U235; ETP-fw = Potential comparative
Toxic Unit for ecosystems; HTP-c = Potential comparative Toxic Unit for humans (cancerogenic); HTP-nc = Potential comparative Toxic Unit for humans
(not cancerogenic); SQP = Potential soil quality index
Disclaimer 1 – for the indicator “Potential Human exposure efficiency relative to U235”.
This impact category deals mainly with the eventual impact of low-dose ionizing radiation on human health of the nuclear fuel cycle. It
does not consider effects due to possible nuclear accidents, occupational exposure or radioactive waste disposal in underground
facilities. Potential ionizing radiation from the soil, radon and from some construction materials is also not measured by this indicator.
Disclaimer 2 – for the indicators “abiotic depletion potential for non-fossil resources”, “abiotic depletion potential for fossil resources”,
“water (user) deprivation potential, deprivation-weighted water consumption”, “potential comparative toxic unit for ecosystems”,
“potential comparative toxic unit for humans – cancerogenic”, “Potential comparative toxic unit for humans - not cancerogenic”,
“potential soil quality index”.
The results of this environmental impact indicator shall be used with care as the uncertainties on these results are high as there is
limited experience with the indicator.
6. LCA: Interpretation
The LCA results of the potential environmental impacts of the consumption is particularly low. All other parameters of the core
ACO gravel grid eco show the highest relevance in fossil indicators follow the scheme with the highest environmental
resource consumption (ADPF) in module A1-A3 with 11.39 MJ impacts in A1-A3 followed by module C3.
and in module C3/1 with 5.51 MJ. The second highest The potential environmental impacts of the ACO gravel grid eco
relevance is the fossil greenhouse potential with 0.544 kg in modules A1-A3 result mainly from the raw material supply of
CO -eq. in modules A1-A3 and 0.532 and 3.43 kg CO -eq. in the PP geotextile from primary material use and the transport of
2 2
modules C3/1 and C3/2, respectively. This is followed by water the raw materials in A2. Electrical energy has a minor impact
consumption with 0.2835 m³ in modules A1-A3 and 0.121 and compared to the raw material supply and the impact is further
0.218 m³ in modules C3/1 and C3/2, respectively. The reduced as green electricity is used in the product system.
relevance of ozone depletion and mineral resource
7. Requisite evidence
Eluate analysis was carried out in accordance with DIN EN 71- - OENORM 5200
3 and DIN EN 62321-3-1. All parameters measured there were - Nordic Countries' Recommendation 2000 7.2 Leaching
below the migration limits (test report ASO-PA B202004). For outer components: Eluate analysis in accordance with DIN
7.1 Radioactivity 38414, Part 4 or the trough method in accordance with the
[Measurement of the nuclide content in Bq/kg for Ra-226, Th- LAGA Directive EW 98 T. The method applied must be
232, K-40. In Germany, there are currently no statutory limit documented.
values specified for assessing the radioactivity of building Measuring agency / Protocol / Date / Result
materials. Assessment can be performed on the basis of the If necessary, explain why this is not relevant.
- EU Commission "Radiation Protection 112" document
8. References
Blue Angel
The Blue Angel (Der Blaue Engel) is the ecolabel of the DIN 16742
German federal government. "Zeichenbenutzungsvertrag Nr. DIN 16742:2013-10, Plastics moulded parts - Tolerances and
35974 zur DE-UZ 30a Ausgabe 2019", label dated 27.08.2021. acceptance conditions
Blue Angel | The German Ecolabel (blauer-engel.de)
DIN EN 1991-1-1-1
Candidate List of SVHC DIN EN 1991-1-1:2010-12, Eurocode 1: Actions on structures -
European Chemicals Agency (ECHA) Candidate List of Part 1-1: General actions - Densities, self-weight, imposed
Substances of Very High Concern (SVHC) for Authorisation loads for buildings; German version EN 1991-1-1:2002 +
https://echa.europa.eu/candidate-list-table (dated 10.06.2022) AC:2009
7 Environmental-Product Declaration - ACO Ahlmann SE & Co. KG - ACO gravel grid eco
Type III environmental declarations — Principles and
DIN EN 62321-3-1 procedures
DIN EN 62321-3-1:2014-10, VDE 0042-1-3-1:2014-10,
Determination of certain substances in electrotechnical ISO 14001
products - Part 3-1: Screening - Lead, mercury, cadmium, total DIN EN ISO 14001:2015-11, Environmental management
chromium and total bromine by X-ray fluorescence systems - Requirements with guidance for use (ISO
spectrometry (IEC 62321-3-1:2013); German version EN 14001:2015)
62321-3-1:2014
ISO 50001
DIN EN 71-3 DIN EN ISO 50001:2018-12, Energy management systems -
DIN EN 71-3:2021-06, Safety of toys - Part 3: Migration of Requirements with guidance for use (ISO 50001:2018)
certain elements; German version
EN 71-3:2019+A1:2021 ISO 9001
DIN EN ISO 9001:2015-11, Quality management systems -
DIN EN ISO 527 Requirements (ISO 9001:2015)
Plastics - Determination of tensile properties - Part 1: General
principles (ISO 527-1:2019) KBA 2020
Kraftfahrtbundesamt, Statistik zur
DIN EN ISO 845 Güterbeförderung, 2020,
DIN EN ISO 845:2009-10, Cellular plastics and rubbers - https://www.kba.de/DE/Statistik/Kraftverkehr/deutscherLastkraftfahrzeuge/vd_Gueterbefoerderung/vd_gueterbefoerderung_node.html
Determination of apparent density (ISO 845:2006)
Ordinance on Biocide Products
EN 15804 European Chemicals Agency (ECHA)
EN 15804:2012+A1:2013, Sustainability of construction works https://echa.europa.eu/regulations/biocidal-products-
— Environmental Product Declarations — Core rules for the regulation/understanding-bpr
product category of construction products https://echa.europa.eu/regulations/biocidal-products-
regulation/legislation (dated 10.06.2022)
EN 15804
EN 15804:2012+A2:2019+AC:2021, Sustainability of PCR Teil A
construction works — Environmental Product Declarations — Institut Bauen und Umwelt e.V., Berlin: Product Category Rules
Core rules for the product category of construction products for Construction Products from the range of Environmental
Product Declarations of Institut Bauen und Umwelt (IBU), Part
EWC A: Calculation Rules for the Life Cycle Assessment and
The European Waste Catalogue, Commission Decision Requirements on the Background Report according to EN
2000/532/EC of the 15804 +A2, version 1.2, 11/2021
European Parliament and of the Council. "Abfallverzeichnis-
Verordnung vom 10. Dezember 2001 (BGBl. I S. 3379), die PCR 2017, Part B
zuletzt durch Artikel 1 der Institut Bauen und Umwelt e.V., Berlin: Product Category Rules
Verordnung vom 30. Juni 2020 (BGBl. I S. 1533) geändert for Construction Products from the range of Environmental
worden ist". Product Declarations of Institut Bauen und Umwelt (IBU), Part
B: Requirements on the EPD for permanent way materials for
IBU 2021 outdoor traffic routes, version 1.6, Institut Bauen und Umwelt e.
General Instructions for the EPD programme of Institut Bauen V., 11/2017
und Umwelt e.V. Version
2.0, Berlin: Institut Bauen und Umwelt e.V., 2021. www.ibu- Software/database
epd.com Software GaBi ts
Database ecoinvent 3, Swiss Center of Life Cycle Inventories,
IEMB 2008 Version 3.6, 2019
Nutzungsdauerangaben von ausgewählten Bauteilen
und Bauteilschichten des Hochbaus für den Leitfaden Test report ASO-PA B202004
'Nachhaltiges Bauen' (Information on the service life of selected Test report ASO-PA
components and component layers in building construction for B202004 according to DIN EN 71-3 and DIN EN 62321-3-1,
the "Sustainable Building" guideline), p. Institute Analytik
113, No. 1299, Institut für Erhaltung und Modernisierung von Service Obernburg ASO, dated 25.11.2020
Bauwerken e. The literature referred to in the Environmental Product
V., TU Berlin (2008) Declaration must be listed in full.Standards already fully quoted
in the EPD do not need to be listed here again.
ISO 14025 The current version of PCR Part A and PCR Part B of the PCR
EN ISO 14025:2011, Environmental labels and declarations — document on which they are based must be referenced.
8 Environmental-Product Declaration - ACO Ahlmann SE & Co. KG - ACO gravel grid eco
Publisher
Institut Bauen und Umwelt e.V. +49 (0)30 3087748- 0
Hegelplatz 1 info@ibu-epd.com
10117 Berlin www.ibu-epd.com
Germany
Programme holder
Institut Bauen und Umwelt e.V. +49 (0)30 3087748- 0
Hegelplatz 1 info@ibu-epd.com
10117 Berlin www.ibu-epd.com
Germany
Author of the Life Cycle Assessment
ACO Ahlmann SE & Co. KG +49 4331 354-0
Am Ahlmannkai - Info@aco.com
24782 Büdelsdorf www.aco.com
Germany
Owner of the Declaration
ACO Ahlmann SE & Co. KG +49 4331 354-0
Am Ahlmannkai - Info@aco.com
24782 Büdelsdorf www.aco.com
Germany
9 Environmental-Product Declaration - ACO Ahlmann SE & Co. KG - ACO gravel grid eco
