ENVIRONMENTAL PRODUCT DECLARATION
as per ISO 14025 and EN 15804+A2
Owner of the Declaration Armacell GmbH
Programme holder Institut Bauen und Umwelt e.V. (IBU)
Publisher Institut Bauen und Umwelt e.V. (IBU)
Declaration number EPD-ARM-20200223-IBB1-EN
Issue date 12.03.2021
Valid to 11.03.2026
AF/ArmaFlex Class O insulation for building equipment and
industrial installations
Armacell GmbH
www.ibu-epd.com | https://epd-online.com
Umwelt Produktdeklaration Name des Herstellers – Name des Produkts
1. General Information
Armacell GmbH AF/ArmaFlex class O
Programme holder Owner of the declaration
IBU – Institut Bauen und Umwelt e.V. Armacell GmbH
Panoramastr. 1 Robert-Bosch-Str. 10
10178 Berlin 48153 Münster - Germany
Germany
Declaration number Declared product / declared unit
EPD-ARM-20200223-IBB1-EN 1m³ insulation material AF/ArmaFlex Class O
This declaration is based on the product Scope:
category rules: Product line AF/ArmaFlex Class O
Insulating materials made of foam plastics, 06.2017 Insulation material for industrial and building
(PCR checked and approved by the SVR) installations vulcanized in tubes and sheets.
This declaration is an Environmental Product
Issue date Declaration according to ISO 14025 describing the
12.03.2021 average environmental performance of the product
produced in Poland and Great Britain.
Valid to The average has been calculated based on site
specific annual production volumes.
11.03.2026
As the installation of the product is not restricted to
countries where the products have been produced the
validity of this EPD is considered at least EU wide.
.
The owner of the declaration shall be liable for the
underlying information and evidence; the IBU shall not
be liable with respect to manufacturer information, life
cycle assessment data and evidences.
The EPD was created according to the specifications
of EN 15804+A2. In the following, the standard will be
simplified as EN 15804.
Verification
The standard EN 15804 serves as the core PCR
Independent verification of the declaration and data
according to ISO 14025:2010
Dipl. Ing. Hans Peters internally x externally
(chairman of Institut Bauen und Umwelt e.V.)
Dr. Alexander Röder Mr Carl-Otto Neven
(Managing Director Institut Bauen und Umwelt e.V.)) (Independent verifier)
2. Product
2.1 Information about the enterprise  Engineered Foams develops high-
Armacell International GmbH is a producer of flexible performance foams for the use in a broad
insulation foams for the equipment insulation market
range of end markets including transportation,
and a provider of engineered foams which operates
automotive, wind energy, sports and
two main businesses:
construction.
 Advanced Insulation develops flexible foams
for the insulation of technical equipment
utilised for the transport of energy - such as The product focus is insulation materials enhancing the
energy efficiency of technical equipment, high-
heating, ventilation & air conditioning (HVAC)
performance foams for technical and lightweight
and heating & plumbing (H&P) in residential
applications, 100% recycled PET products and next-
and commercial construction, process lines in
generation aerogel technology.
the heavy- and oil & gas industry, equipment
in transportation, as well as, acoustics.
2 Environmental Product Declaration Armacell GmbH – AF/ArmaFlex Class O insulation for industrial and building
installation
2.2 Product description/Product definition normal building moisture does not lead to an increase
AF/ArmaFlex Class O is the professional, highly- in thermal conductivity.
flexible, closed-cell elastomeric foam insulation (FEF)
for continuous energy saving and condensation control Performance data of the product in accordance with
purposes. The combination of very low thermal the declaration of performance with respect to its
conductivity and extremely high resistance to water essential characteristics according to EN 14304:2013-
vapour transmission prevents long-term energy losses 04.
and water vapour ingress and reduces the risk of
corrosion under insulation. 2.5 Delivery status
FEF made of cross-linked elastomer is supplied as
For the placing on the market of the product in sheets, tubes and shaped pieces. Products with self-
the European Union/European Free Trade Association adhesive backings/closures are available; these
(EU/EFTA) (with the exception of Switzerland) variations are not included in the calculations.
Regulation (EU) No. 305/2011 (CPR) applies. The Insulation thicknesses are available for all common
product needs a declaration of performance taking into pipe diameters up to an outer diameter of 114 mm
consideration EN 14304:2013-04: Thermal insulation (tubes).
products for building equipment and industrial
installations – Factory made flexible elastomeric foam 2.6 Base materials/Ancillary materials
(FEF) products – Specification and the CE-marking.
For the application and use the respective national ArmaFlex is a highly flexible insulation material based
provisions apply. on synthetic rubber, which consists of around 20 basic
components. The following table displays the
2.3 Application composition split into functional substance groups.
AF/ArmaFlex Class O is used to insulate pipes, air
ducts and vessels including fittings and flanges of Name Value Unit
industrial installations and building equipment. Rubber and polymers 24 %
 Condensation control, energy saving and Fillers and pigments 3 %
noise control in refrigeration and air Blowing agent 13 %
conditioning equipment and process plants. Vulcanisation system, additives, 37 %
plasticisers
 Energy saving according to local energy-
Flame retardant 23 %
saving laws, prevention of heat loss and noise
reduction of heating and plumbing systems.
Synthetic rubber determines the flexibility;
 Condensation control and noise reduction in Fillers determine the fire properties and firmness;
service-water and waste-water systems. Blowing agent causes the expansion process during
 Condensation control, energy saving and manufacturing;
Accelerator and sulphur enable the vulcanisation;
noise control in refrigeration and air-
Plasticizers determine the flexibility;
conditioning equipment in the ship-building
Flame retardants ensure fire resistance.
sector.
According to the European Chemicals Regulation
REACH manufacturer, importers and downstream
2.4 Technical Data users must register their chemicals and are
responsible for their safe use on their own. For its
production Armacell uses exclusively verifiably
Constructional data registered and approved substances / mixtures.
Name Value Unit According to available data and the information
Gross density 52.5 kg/m3 provided by preliminary suppliers, the product does not
Water vapour diffusion resistance contain substances (SVHC) that are considered
≥ 10000/ ≥
factor acc. to EN 12086, EN - substances meeting the criteria for inclusion in annex
7000
13469 XIV (List of Substances Subject to Authorisation) as
0,033/0,03 laid down in Article 57 and article 59 of REACH (EC)
Thermal conductivity 6 (0°C) W/(mK) 1907/2006.). Products manufactured and marketed by
Armacell do not have to be registered. The products
Maximum service temperature
+110 °C may contain traces of azodicarbonamide (ACDA).
acc. to EN 14706, EN 14707
Possible minimal residual amounts are included in the
Minimum service temperature -50 °C
polymer matrix. A health impairment can be excluded.
Tubes: BL-
For the production of insulation material based on
Reaction to fire acc. to EN 13501- s3, d0/
- synthetic rubber, there is presently no alternative to
1 Sheets: B-
ADCA available.
s3, d0
Armaflex class O is treated with the antimicrobial
Structure-borne sound
not biocide pyrithione zinc.
transmission acc. to EN ISO
relevant
3822-1
Weighted sound absorption
not 2.7 Manufacture
coefficient αw acc. to EN ISO
relevant ArmaFlex products are manufactured in a
11654
pressureless, continuous and discontinuous production
process.
Insulation materials on the basis of synthetic rubber do
In the first step, a homogenous compound is produced
not absorb moisture from the air. For this reason the
with rubber, additives, ancillary materials, blowing and
3 Environmental Product Declaration Armacell GmbH – AF/ArmaFlex Class O insulation for industrial and building
installation
vulcanization agents. This is done on the rolling mill or determined after consideration of real life applications
in the internal mixer followed by the rolling mill. with FEF products (in living rooms) and
Rubber extruders are used to process the compounds recommendation of experts of the test institute, all
to produce raw profiles with defined dimensions. Here results were clearly below the limit values. For
exact compliance with the dimensions for the raw example, the determined total volatile organic
profile is crucial for the dimensional accuracy of the compound (TVOC) after 28 days was for all samples
foamed product. below 100 mg/m3. Certificates are available on
In the case of the discontinuous, pressureless request.
production process, the raw profiles are cut to length
and then foamed in a hot-air oven. In the case of the
continuous, pressureless process, the extruded profile 2.13 Reference service life
is fed directly onto a vulcanization line whose energy ArmaFlex products are long-lasting products. Findings
source may be hot air, for example. show that when used and installed properly they can
In foam production, vulcanization and blowing have an estimated service life of more than 50 years. It
processes run alongside each other. Both reactions is practically only restricted by the service life of the
are regulated by temperature control. Recipe and equipment or whole building, which can extent that
temperature control determine the properties of the time period. The insulation performance is almost
foam. completely maintained over the entire service life. The
Quality assurance: insulation performance is only compromised by
EC Certificate of conformity no. 0543 of the extraordinary impacts and damage during construction.
Gütegemeinschaft Hartschaum e.V. Celle.
Quality management system in accordance with EN
ISO 9001. 2.14 Extraordinary effects
2.8 Environment and health during Fire
manufacturing According to EN 13501, ArmaFlex is classified as a
During all manufacturing steps and at all production combustible insulation material. Due to its material
sites of Armacell, the production follows the national structure ArmaFlex does not contribute to an
guidelines and regulations. A regenerative thermal uncontrollable spread of fire under installation
oxidizer is installed to treat exhaust air. conditions typical on a building site. ArmaFlex does not
Certification of the environmental management system drip under practical fire conditions, this means that fire
is in accordance with ISO 14001. spread is ruled out. The product is self-extinguishing
and therefore only makes a minor contribution to the
actual fire event. There is no possibility of the material
2.9 Product processing/Installation self-igniting. ArmaFlex does not propagate the fire
The product is installed by using knives. No special either horizontally or vertically.
tools, nor specific protection is necessary.
When applying adhesives the information given in the Fire protection
relevant safety data sheets is to be heeded. Name Value
The recommendations for installing the product Tubes: BL
depend on the product and system and are described Euro class / Sheets:
in the respective documents (e.g. Armaflex application B
manual) and on the data sheets. More details under Tubes/She
Burning droplets
www.armacell.com. ets: d0
Tubes/She
Smoke development
ets: s3
2.10 Packaging
As a rule, ArmaFlex products are packaged in Water
cardboard boxes and transported on reusable pallets. Armacell insulation materials have a high resistance to
Over-sized rolls of sheet material are packaged in water vapour transmission which keeps possible water
polyethylene (PE) foil. The cardboard boxes can be vapour transmission processes to a minimum
recycled through Interseroh’s dual system. permanently. Therefore, a significant reduction in the
insulation effect can be ruled out permanently.
If the insulation material is exposed to water over a
2.11 Condition of use long period of time (e.g. flooding) it should be replaced.
When the products are used for the purpose for which
they are intended, there are no changes in the material Mechanical destruction
composition during use, except in the event of ArmaFlex insulation materials are flexible foams and
extraordinary impacts (see 2.14). thus display limited mechanical stability. Therefore, if
the material will be subject to greater mechanical
2.12 Environment and health during use impact it should be protected appropriately, e.g. by a
Ingredients: There are no particular aspects of the metal jacket or Arma-Chek covering.
material composition during use. ArmaFlex products (with the exception of
Eurofins Product Testing A/S has tested a wide range HT/ArmaFlex) are not UV resistant. If the material is
and varieties of typical FEF (Flexible Elastomeric subject to UV-rays it should be protected accordingly.
Foam) products marketed in the EU from CEFEP
(European Group of FEF manufacturers). Sampling, 2.15 Re-use phase
testing and evaluation were performed according to If removed properly the product can be re-used.
CEN TS 16516, AgBB, ISO 16000-3, ISO 16000-6, Correctly sorted material can be ground and used to
ISO 16000-9, ISO 16000-11 in the latest versions. manufacture new products (e.g. ArmaSound).
Based on the loading factor 0.05 m²/m³, which was
4 Environmental Product Declaration Armacell GmbH – AF/ArmaFlex Class O insulation for industrial and building
installation
2.16 Disposal 2.17 Further information
Dispose of the materials according to local regulations. Further information on ArmaFlex® can be found on the
Regulated by the European Waste Catalogue: Waste manufacturer’s website www.armacell.com. Detailed
code 07 02 13 (waste plastic). specification clauses for the products are provided at
Note: Please observe Commission Decision www.armaflex.de.
2001/118/EC.
3. LCA: Calculation rules
3.1 Declared Unit product can be joined; thus installation off-cut is very
The declaration refers to 1 m³ insulation product. small. A loss of 1% is assumed.
For the LCA calculations the average density per Transport to customer (A4):
product brand is used. Armacell’s data collectors reported average figures for
As additional information and support for installers the the distribution of their material. Depending on the
thermal conductivity coefficient (lambda-value) and R- country, the transport distance varies from 500 km to
value per 20 cm thickness per product brand are given. 800 km
End-of-life (C2, C3):
Declared unit The transport from place of usage to a waste
Name Value Unit incineration plant is assumed as 100 km.
Declared unit 1 m3 After the demolition of the product a current realistic
Gross density 52.5 kg/m3 End-of-life scenario is the incineration of the material.
Conversion factor to 1 kg 52.5 - According to the reported net calorific value of the
materials and the elementary composition, a partial
Thermal conductivity λ : 0.033 W/(mK (0°C) stream consideration for the incineration process of
R-value – thickness: 20 cm: 6.1 (m²K)/W PVC-products is applied as an approximation for all
declared products.
Inventory estimations and approximations:
The reported recipes for the rubber mixes contain
3.2 System boundary specific substances of the rubber industry. For these
The data collection refers to the yearly production in materials only partly life cycle inventories are available.
2019. The following life cycle stages are considered: Approximations are used with the consideration of
similar supply chain effort or similar elementary
Type of EPD: Cradle-to-Gate with options: composition. Partly an estimation is modelled using
pre-products of the specific material and adding an
Production A1-A3: energy effort as well as considering the treatment of
The LCA calculation covers the production of the raw production residues for this step in the supply chain.
materials (supply chain – A1), the mixing of raw
materials according to the respective recipes 3.4 Cut-off criteria
(MasterBatch) exclusively done in Münster, Germany, In the assessment, all reported data from the
the transport (A2) of the MasterBatches to the production process are considered, utilised thermal
production facility for foaming and the foaming process energy, and electric power consumption using best
(A3) in Germany, Spain, Poland or Great Britain, available life cycle inventory (LCI) datasets. Thus
including the packaging material. material and energy flows contributing less than 1% of
Transport A4: mass or energy are considered.
Average values for the transport from factory gate to No cut-off criteria are applied in the foreground data in
construction site are assumed. this study.
Installation A5: For cut-off criteria in the background system, see
The installation considers the production of off-cuts, information provided in the modelling principles and
incineration of these off-cuts and the disposal scenario specific documentations (documentation.gabi-
for the packaging material. Auxiliaries like adhesives or software.com).
tapes or energy for installation are not considered.
End-of-life C2, C3: 3.5 Background data
An incineration scenario for the used and demolished The LCA model is created using the GaBi ts Software
product, including an assumption for the transport to system (v9) for life cycle engineering, developed by
disposal, is covered. Sphera. The GaBi LCI database provides the life cycle
Benefits for the next product system D: inventory data for several of the raw and process
Credits for electrical and thermal energy resulting from materials obtained from the background system. The
the waste incineration process of the off-cut material most recent update of the database was 2020.
and packaging (A5) and the product (C3) are declared
in module D. 3.6 Data quality
The foreground data collected by the manufacturer are
based on yearly production amounts and
3.3 Estimates and assumptions extrapolations of measurements on specific machines
Scenario assumptions: and plants. As the average environmental performance
Installation (A5): of the product brand has been calculated by a
The additional demand of material for installation weighting of the site-specific production volumes the
depends on the specific frame conditions of the results also show a representative picture regarding
building and pipe system to be insulated. Parts of the site specific production technologies. The average
results therefore can be assessed as robust.
5 Environmental Product Declaration Armacell GmbH – AF/ArmaFlex Class O insulation for industrial and building
installation
Most of the necessary life cycle inventories for the energy from the incineration process is looped inside
basic materials are available in the GaBi database. module A1-A3. The quality of the recovered energy is
The last update of the database was in 2020 (service assumed to the same as that of the input energy.
pack 40). Landfilling of plastic material is assumed not to deliver
Further LCIs for materials of the supply chain of the any landfill gas.
basic materials are approximated with LCIs of similar All applied incineration processes are displayed via a
materials or estimated by the combination of available partial stream consideration for the combustion
LCIs. process, according to the specific composition of the
For electrical and thermal energy regional specific grid incinerated material. For the waste incineration plant
mixes and regional specific supply for natural gas are an R1-value of > 0.6 is assumed.
considered. Environmental burden of the incineration of installation
residues (off-cuts), packaging and the product in the
3.7 Period under review end-of-life scenario are assigned to the system (A5 or
The production data refer to an average of the year C3); resulting credits for thermal and electrical energy
2019. are declared in module D.
The credits for thermal and electrical energy are
3.8 Allocation calculated via inversion of the life cycle inventory of
Allocation of upstream data: European average data.
For all refinery products, allocation by mass and net Allocation for waste paper:
calorific value is applied. The specific manufacturing Paper/corrugated board is used as packaging material
route of every refinery product is modelled and so the and this usually includes a mix of recycled and virgin
impacts associated with the production of these fibres. When modelling the production of paper, the
products are calculated individually. scrap paper that is used in this process has been
Materials and chemicals used in the manufacturing assumed to be burden free. Similarly, waste paper
process are modelled using the allocation rule most arising in the product life cycle is assumed to be
suitable for the respective product. For further recycled. Robust data on paper and cardboard
information on a specific product see recycling are not promptly available and refer to a very
documentation.gabi-software.com. complex system. Hence, to apply this methodology
Allocation in the foreground data: consistently throughout the model, a cut-off approach
Part of the production residues (ca. 2%) are used for has been applied, i.e., input of waste paper is
the manufacturing of a non-declared product considered without environmental burden, resulting
(ArmaSound). These materials leave the process waste paper is not credited. The recycling process and
without further consideration of any treatment and the production process of paper are merged in the
without credit (cut-off-approach). production process. The C-balance referring to fresh
No further allocation is applied in the software model. fibre is corrected via CO2 emissions (biotic)
The overall production of the Armacell production (assumption of final rotting or incineration in the time
facilities comprises further products beside the frame of 100 years).
products considered in this study. Data for thermal and
electrical energy, as well as auxiliary material, refer to 3.9 Comparability
the declared products only. During data collection the Basically, a comparison or an evaluation of EPD data
allocation is done via mass, area, pieces or time spent is only possible if all the data sets to be compared
in the machine, depending on the process step and were created according to EN 15804 and the building
reasonable split. The data collectors at Armacell context, respectively the product-specific
decided on the distribution basis. characteristics of performance, are taken into account.
Allocation for waste materials:
Production waste is sent to a waste incineration plant The used background dataset DB has been GaBi
and to landfill (Spain). Resulting electrical and thermal (service pack. 40, 2020).
4. LCA: Scenarios and additional technical information
Characteristic product properties Biogenic Carbon Content in
29.19 kg C
Information on biogenic Carbon accompanying packaging
The biogenic carbon content quantifies the amount of The embodied biogenic carbon leaves the system in
biogenic carbon in a construction product leaving the Module A5
factory gate, and it shall be separately declared for the
product and any accompanying packaging.If the total The following technical information serves as basis for
mass of biogenic carbon containing materials is less the declared modules. The values refer to the declared
than 5 % of the total mass of the product and unit of 1 m³.
accompanying packaging, the declaration of biogenic
carbon content may be omitted. The mass of Transport to the building site (A4)
packaging containing biogenic carbon shall always be Name Value Unit
declared. Litres of fuel 0.14 l/100km
Note: 1 kg biogenic Carbon is equivalent to 44/12 kg of 253 -
Transport distance km
CO2 500
Capacity utilisation (including empty
85 %
Information on describing the biogenic Carbon runs)
Content at factory gate
Name Value Unit Installation into the building (A5)
Biogenic Carbon Content in 0 kg C Name Value Unit
product Material loss 1 %
6 Environmental Product Declaration Armacell GmbH – AF/ArmaFlex Class O insulation for industrial and building
installation
Reference service life
Name Value Unit
Life Span according to the
50 a
manufacturer
End of life (C1-C4)
Name Value Unit
Energy recovery in WIP 52,5 kg
Reuse, recovery and/or recycling potentials (D),
relevant scenario information
Module D includes the credits of the incineration
processes from A5 (off-cut of product installation,
packaging waste) and C3 (incineration of the product).
A waste incineration plant with an R1-value > 0.6 is
assumed.
7 Environmental Product Declaration Armacell GmbH – AF/ArmaFlex Class O insulation for industrial and building
installation
5. LCA: Results
The following information on environmental impacts is expressed with the impact category parameters of LCIA
using characterisation factors. The chosen characterisation factors fulfil the requirements of EN 15804.
Disclaimer:
EP-freshwater: This indicator has been calculated as “kg P eq” as required in the characterization model
(EUTREND model, Struijs et al., 2009b, as implemented in ReCiPe;
http://eplca.jrc.ec.europa.eu/LCDN/developerEF.xhtml)
DESCRIPTION OF THE SYSTEM BOUNDARY (X = INCLUDED IN LCA; ND = MODULE OR INDICATOR NOT
DECLARED; MNR = MODULE NOT RELEVANT)
BENEFITS AND
CONSTRUCTI LOADS
PRODUCT STAGE ON PROCESS USE STAGE END OF LIFE STAGE BEYOND THE
STAGE SYSTEM
BOUNDARIES
8 Environmental Product Declaration Armacell GmbH – AF/ArmaFlex Class O insulation for industrial and building
installation
lairetam
waR
ylppus tropsnarT
gnirutcafunaM
eht
morf
tropsnarT
etis
eht
ot
etag
ylbmessA esU
ecnanetniaM
riapeR
tnemecalpeR tnemhsibrufeR
ygrene
lanoitarepO esu
retaw
lanoitarepO esu
noitcurtsnoc-eD
noitilomed tropsnarT
gnissecorp
etsaW
lasopsiD -esueR -yrevoceR -gnilcyceR laitnetop
A1 A2 A3 A4 A5 B1 B2 B3 B4 B5 B6 B7 C1 C2 C3 C4 D
X X X X X ND ND MNR MNR MNR ND ND ND X X ND X
RESULTS OF THE LCA - ENVIRONMENTAL IMPACT according to EN 15804+A2: 1 m³ AF/ArmaFlex Class
O insulation for industrial and building installation
Core Indicator Unit A1-A3 A4 A5 C2 C3 D
Global warming potential - total [kg CO2-Eq.] 1.65E+2 1.10E+0 6.46E+1 2.50E-1 1.36E+2 -3.85E+1
Global warming potential - fossil fuels [kg CO2-Eq.] 2.21E+2 1.10E+0 5.04E+0 2.49E-1 1.36E+2 -3.84E+1
Global warming potential - biogenic [kg CO2-Eq.] -5.69E+1 -1.87E-3 5.95E+1 -4.25E-4 -5.95E-2 -9.00E-2
GWP from land use and land use change [kg CO2-Eq.] 4.13E-1 8.87E-3 4.66E-3 2.02E-3 2.77E-2 -2.68E-2
Depletion potential of the stratospheric ozone layer [kg CFC11-Eq.] 1.24E-9 1.32E-16 1.27E-11 2.99E-17 2.07E-13 -3.99E-13
Acidification potential, accumulated exceedance [mol H+-Eq.] 1.24E+0 3.28E-3 1.53E-2 7.46E-4 4.05E-2 -5.36E-2
Eutrophication, fraction of nutrients reaching freshwater
end compartment
[kg PO4-Eq.] 2.25E-3 3.33E-6 2.32E-5 7.56E-7 3.49E-5 -4.93E-5
Eutrophication, fraction of nutrients reaching marine end
[kg N-Eq.] 1.62E-1 1.46E-3 2.46E-3 3.32E-4 1.34E-2 -1.39E-2
compartment
Eutrophication, accumulated exceedance [mol N-Eq.] 1.58E+0 1.64E-2 2.80E-2 3.72E-3 1.64E-1 -1.49E-1
Formation potential of tropospheric ozone photochemical
[kg NMVOC-Eq.] 3.67E+0 2.89E-3 3.94E-2 6.56E-4 3.79E-2 -3.99E-2
oxidants
Abiotic depletion potential for non-fossil resources [kg Sb-Eq.] 4.11E+3 1.46E+1 4.73E+1 3.31E+0 2.51E+2 -6.51E+2
Abiotic depletion potential for fossil resources [MJ] 1.20E+0 7.85E-8 1.24E-2 1.78E-8 2.98E-6 -6.28E-6
Water (user) deprivation potential, deprivation-weighted [m³ world-Eq
2.67E+1 9.79E-3 1.97E+0 2.22E-3 1.05E+1 -3.96E+0
water consumption (WDP) deprived]
RESULTS OF THE LCA - INDICATORS TO DESCRIBE RESOURCE USE according to EN 15804+A2: 1 m³
AF/ArmaFlex Class O insulation for industrial and building installation
Indicator Unit A1-A3 A4 A5 C2 C3 D
Renewable primary energy as energy carrier [MJ] 1.30E+3 8.20E-1 1.17E+2 1.86E-1 5.21E+1 -1.42E+2
Renewable primary energy resources as material utilization [MJ] 1.02E+2 0.00E+0 -1.02E+2 0.00E+0 0.00E+0 0.00E+0
Total use of renewable primary energy resources [MJ] 1.40E+3 8.20E-1 1.52E+1 1.86E-1 5.21E+1 -1.42E+2
Non-renewable primary energy as energy carrier [MJ] 3.20E+3 1.46E+1 6.85E+1 3.32E+0 1.15E+3 -6.51E+2
Non-renewable primary energy as material utilization [MJ] 9.19E+2 0.00E+0 -2.11E+1 0.00E+0 -8.98E+2 0.00E+0
Total use of non-renewable primary energy resources [MJ] 4.12E+3 1.46E+1 4.74E+1 3.32E+0 2.51E+2 -6.51E+2
Use of secondary material [kg] 3.54E+1 0.00E+0 0.00E+0 0.00E+0 0.00E+0 0.00E+0
Use of renewable secondary fuels [MJ] 0.00E+0 0.00E+0 0.00E+0 0.00E+0 0.00E+0 0.00E+0
Use of non-renewable secondary fuels [MJ] 0.00E+0 0.00E+0 0.00E+0 0.00E+0 0.00E+0 0.00E+0
Use of net fresh water [m³] 1.53E+0 9.49E-4 5.56E-2 2.16E-4 2.76E-1 -1.64E-1
RESULTS OF THE LCA – WASTE CATEGORIES AND OUTPUT FLOWS according to EN 15804+A2:
1 m³ AF/ArmaFlex Class O insulation for industrial and building installation
Indicator Unit A1-A3 A4 A5 C2 C3 D
Hazardous waste disposed [kg] 2.39E-5 6.79E-7 2.64E-7 1.54E-7 1.14E-6 -2.59E-7
Non-hazardous waste disposed [kg] 1.18E+1 2.23E-3 1.18E+0 5.08E-4 8.35E+1 -3.00E-1
Radioactive waste disposed [kg] 1.25E-1 1.81E-5 1.51E-3 4.11E-6 7.97E-3 -4.84E-2
Components for re-use [kg] 0.00E+0 0.00E+0 0.00E+0 0.00E+0 0.00E+0 0.00E+0
Materials for recycling [kg] 0.00E+0 0.00E+0 2.92E+1 0.00E+0 0.00E+0 0.00E+0
Materials for energy recovery [kg] 0.00E+0 0.00E+0 0.00E+0 0.00E+0 0.00E+0 0.00E+0
Exported electrical energy [MJ] 0.00E+0 0.00E+0 2.32E+1 0.00E+0 1.37E+2 0.00E+0
Exported thermal energy [MJ] 0.00E+0 0.00E+0 4.17E+1 0.00E+0 2.50E+2 0.00E+0
RESULTS OF THE LCA – additional impact categories according to EN 15804+A2-optional:
1 m³ AF/ArmaFlex Class O insulation for industrial and building installation
Indicator Unit A1-A3 A4 A5 C2 C3 D
Potential incidence of disease due to PM emissions [Disease
7.17E-5 1.82E-8 7.63E-7 4.13E-9 9.74E-7 -4.55E-7
Incidence]
Potential Human exposure efficiency relative to U235 [kBq U235-
1.28E+1 2.61E-3 1.66E-1 5.94E-4 8.09E-1 -7.93E+0
Eq.]
Potential comparative toxic unit for ecosystems [CTUe] 4.69E+3 1.03E+1 4.86E+1 2.34E+0 2.08E+2 -1.40E+2
Potential comparative toxic unit for humans - cancerogenic [CTUh] 8.36E-8 2.16E-10 1.04E-9 4.90E-11 8.23E-9 -6.08E-9
Potential comparative toxic unit for humans - not cancerogenic [CTUh] 1.15E-5 1.26E-8 1.31E-7 2.85E-9 8.75E-7 -2.26E-7
Potential soil quality index [-] 4.10E+3 5.12E+0 4.28E+1 1.16E+0 5.70E+1 -1.02E+2
Disclaimer 1 – for the indicator IRP
This impact category deals mainly with the eventual impact of low dose ionizing
radiation on human health of the nuclear fuel cycle. It does not consider effects due to possible
nuclear accidents, occupational exposure nor due to radioactive waste disposal in underground
facilities. Potential ionizing radiation from the soil, from radon and from some construction materials is also not
measured by this indicator.
Disclaimer 2 – for the indicators ADPE, ADPF, WDP, ETP-fw, HTP-c, HTP-nc, SQP
The results of this environmental impact indicator shall be used with care as the
uncertainties on these results are high or as there is limited experienced with the indicator.
6. LCA: Interpretation
The supply chain, i.e. the production of the purchased the overall green house gas emissions. At the same
materials, causes the highest influence on all impact time a credit (D) of 12% is given to the next system,
categories and the primary energy. due to the use of electrical and thermal energy, gained
in the incineration processes for the product and the
Global Warming Potential off-cut material.
Looking at the GWP for the overall declared life cycle
phases, including production (A1-A3), transport (A4, Further impact categories
C2), installation (losses) (A5) and end-of-life (C3, D), The end-of-life scenarios have less influence on the
the production (A1-A3) contributes to 50%. other considered impact categories than on GWP. The
The production in the supply chain (A1) already main contribution of the considered life cycle phases is
contributes 50% to the total GWP value. Thus, every concentrated on module A1-A3.
increase in the production yield directly improves the The energy consumption in the foaming step
environmental performance of the products. influences all impact categories; variations depend on
The foaming process (A3), which includes the the national grid mixes for electricity.
electrical and thermal energy for the mixing, the
vulcanisation and blowing step as well as the Primary Energy Demand
production of the packaging materials, shows a The total primary energy demand is for both categories
significant influence on GWP of the life cycle with (renewable and non-renewable) significantly (> 100%)
0.22%. influenced by the production of the module A1-A3. The
Module A5 covers the production and disposal other modules play a minor role (C3 with about 6%)
(=incineration) of the off-cut material assumed as 1%
loss in respect to the required insulation material. The share of primary energy bound as material
Additionally, the emissions of the incineration of accounts for about 20%, which is partly recovered and
packaging material (plastic, wood) in a waste credited for in module D (-16%)
incineration plant are considered. The installation step
contributes with 20% to the overall GWP.
As end-of-life scenario an incineration is considered.
The emissions of the product (C3) contribute to 41% to
7. Requisite evidence
recommendation of the experts of the test institute, all
7.1 VOC emissions results were clearly below the limit values. For
Eurofins Product Testing A/S has tested a wide range example the determined TVOC after 28 days was for
and varieties of typical FEF (Flexible Elastomeric all samples below 100 mg/m3. Certificates are
Foam) products marketed in the EU from CEFEP available on request.
(European Group of FEF manufacturers). Sampling,
testing and evaluation were performed according to 7.2 Leaching performance
CEN TS 16516, AgBB, ISO 16000-3, ISO 16000-6, According to EN 13468 is the content of water-soluble
ISO 16000-9, ISO 16000-11 in the latest versions. chloride ions for AF/Armaflex Class O ≤ 300 ppm.
Based on the loading factor 0.05 m²/m³, which were
determined after consideration of real life applications
with FEF products (in living rooms) and
9 Environmental Product Declaration Armacell GmbH – AF/ArmaFlex Class O insulation for industrial and building
installation
8. References
AgBB building equipment and industrial installations -
Umweltbundesamt Germany, Health-related Determination of maximum service temperature
Evaluation of Emissions of Volatile Organic
Compounds (VVOC, VOC and SVOC) from Building EN 14707
Products EN 14707: 2013-01: Thermal insulating products for
building equipment and industrial installations -
CEFEP Determination of maximum service temperature for
The industry association for FEF and PEF insulation preformed pipe insulation
(Celle) in 2012
EN 15801
CEN TS 16516 EN 15801: 2010-04: Conservation of cultural property -
CEN TS 16516:2013-12: Construction products - Test methods - Determination of water absorption by
Assessment of release of dangerous substances - capillarity
Determination of emissions into indoor air
EN 15804
Comission Decision 2001/118/EC EN 15804:2012-04+A1 2013, Sustainability of
Amendment to European Waste Catalogue construction works — Environmental Product
Declarations — Core rules for the product category of
CPR construction products.
Regulation (EC) No 305/2011, Construction Products
Regulation EN 15804
EN 15804:2019+A2 (in press), Sustainability of
EN 826 construction works — Environmental Product
EN 826: 2013-05: Thermal insulating products for Declarations — Core rules for the product category of
building applications - Determination of compression construction products.
behaviour
EN 29052
EN 1606 EN 29052: 1992-08: Acoustics; determination of
EN 1606: 2013-05: Thermal insulating products for dynamic stiffness; part 1: materials used under floating
building applications - Determination of compressive floors in dwellings
creep
EU/EFTA
EN 12091 Regulation (EU) No. 305/2011 (CPR), European
EN 12091: 2013-06: Thermal insulating products for Union/European Free Trade Association (EU/EFTA)
building applications - Determination of freeze-thaw
resistance Eurofins Product Testing A/S
Eurofins Miljo, Smedeskowej 38, 8464 Galten,
EN 12086 Denmark
EN 12086:2013-06: Thermal insulating products for
building applications - Determination of water vapour European Waste Catalogue
transmission properties European Waste Catalogue and Hazardous Waste
List, Commission Decision 2000/532/EC
EN 13468
EN 13468: 2001-12: Thermal insulating products for GaBi
building equipment and industrial installations - GaBi 9 software-system and databases, LBP,
Determination of trace quantities of water soluble University of Stuttgart and Sphera, Leinfelden-
chloride, fluoride, silicate, and sodium ions and pH Echterdingen, 2020 (http://documentation.gabi-
software.com/)
EN 13469
EN 13469:2013-01: Thermal insulating products for IBU
building equipment and industrial installations - Institut Bauen und Umwelt e.V.: General Programme
Determination of water vapour transmission properties Instructions for the Preparation of EPDs at the Institut
of preformed pipe insulation Bauen und Umwelt e.V. Version 1., Berlin: Institut
Bauen und Umwelt e.V., 2016. www.ibu-epd.com
EN 13501-1
EN 13501-1: 2010-01: Fire classification of IBU PCR Part A
construction products and building elements - Part 1: PCR - Part A: Calculation Rules for the Life Cycle
Classification using data from reaction to fire tests Assessment and Requirements on the Project Report,
Institut Bauen und Umwelt e.V., www.ibu-epd.com,
EN 14304 2019.
EN 14304:2013-04: Thermal insulation products for
building equipment and industrial installations – IBU PCR PART B
Factory made flexible elastomeric foam (FEF) products PCR – Part B: Requirements on the EPD for Insulation
– Specification materials made of foam plastics, version 1.7, 01-2019 ,
Institut Bauen und Umwelt e.V., www.ibu-epd.com,
EN 14706 2019
EN 14706: 2013-01: Thermal insulating products for
10 Environmental Product Declaration Armacell GmbH – AF/ArmaFlex Class O insulation for industrial and building
installation
ISO 3822-1 ISO 16000-11
ISO 3822-1: 1999-05: Acoustics - Laboratory tests on ISO 16000-11: 2006-02: Indoor air - Part 11:
noise emission from appliances and equipment used in Determination of the emission of volatile organic
water supply installations - Part 1: Method of compounds from building products and furnishing -
measurement Sampling, storage of samples and preparation of test
specimens
ISO 9001
ISO 9001:2014-08: Quality management systems – ISO 16000-3
Requirements ISO 16000-3:2011-10: Determination of formaldehyde
and other carbonyl compounds in indoor air and test
ISO 11654 chamber air - Active sampling method
ISO 11654: 1997-04: Acoustics - Sound absorbers for
use in buildings - Rating of sound absorption ISO 16000-6
ISO 16000-6:2011-12: Indoor air - Part 6:
ISO 14001 Determination of volatile organic compounds in indoor
ISO 14001:2015, Environmental management systems and test chamber air by active sampling on Tenax TA®
— Requirements with guidance for use sorbent, thermal desorption and gas chromatography
using MS or MS-FID
ISO 14025
ISO 14025:2011-10, Environmental labels and ISO 16000-9
declarations — Type III environmental declarations — ISO 16000-9:2006-02: Indoor air - Part 9:
Principles and procedures. Determination of the emission of volatile organic
compounds from building products and furnishing -
ISO 14040 Emission test chamber method
ISO 14040:2009-11: Environmental management –
Life cycle assessment – Principles and framework
REACH
ISO 14044 Regulation (EC) No 1907/2006, Regulation concerning
ISO 14044:2006-10: Environmental management – the Registration, Evaluation, Authorisation and
Life cycle assessment – Requirements and guidelines Restriction of Chemicals (REACH)
ISO 15868
ISO 15686:2011-05, Buildings and constructed assets
- Service life planning
11 Environmental Product Declaration Armacell GmbH – AF/ArmaFlex Class O insulation for industrial and building
installation
Publisher
Institut Bauen und Umwelt e.V. Tel +49 (0)30 3087748- 0
Panoramastr. 1 Fax +49 (0)30 3087748- 29
10178 Berlin Mail info@ibu-epd.com
Germany Web www.ibu-epd.com
Programme holder
Institut Bauen und Umwelt e.V. Tel +49 (0)30 - 3087748- 0
Panoramastr 1 Fax +49 (0)30 – 3087748 - 29
10178 Berlin Mail info@ibu-epd.com
Germany Web www.ibu-epd.com
Author of the Life Cycle
Assessment Tel +49 711 341817-0
Sphera Solutions GmbH Fax +49 711 341817-25
Hauptstraße 111- 113 Mail info@sphera.com
70771 Leinfelden-Echterdingen Web http://www.sphera.com
Germany
Owner of the Declaration
Armacell GmbH Tel +49-251-7603-0
Robert-Bosch-Str. 10 Fax +49-251-7603-346
48153 Münster Mail info.de@armacell.com
Germany Web www.armacell.de
