ENVIRONMENTAL PRODUCT DECLARATION
as per ISO 14025 and EN 15804+A2
Owner of the Declaration European Association for Panels and Profiles e. V. (PPA-Europe)
Publisher Institut Bauen und Umwelt e.V. (IBU)
Programme holder Institut Bauen und Umwelt e.V. (IBU)
Declaration number EPD-PPA-20240130-CBG2-EN
Issue date 19.07.2024
Valid to 18.07.2029
Profiled sheets made of aluminium for roof, wall and ceiling
constructions
PPA-Europe
www.ibu-epd.com | https://epd-online.com
General Information
PPA-Europe Profiled sheets made of aluminium for roof, wall
and ceiling constructions
Programme holder Owner of the declaration
IBU – Institut Bauen und Umwelt e.V. European Association for Panels and Profiles e. V. (PPA-Europe)
Hegelplatz 1 Europark Fichtenhain A 13a
10117 Berlin 47807 Krefeld
Germany Germany
Declaration number Declared product / declared unit
EPD-PPA-20240130-CBG2-EN 1m² industrially produced aluminium profiled sheets
This declaration is based on the product category rules: Scope:
Thin walled profiles and profiled panels of metal, 01.08.2021 This document is an association EPD for 1 m² aluminium trapezoidal
(PCR checked and approved by the SVR) 35/207 profile and it represents an average EPD, based on vertical
averaging of the specific producer datasets under consideration of the
yearly production amounts. Its applicability is limited to aluminium profiled
Issue date sheets, which are manufactured by member companies of the European
Association for Panels and Profiles.
19.07.2024
The following member companies of the European Association for Panels
and Profiles have provided data for the year 2022:
Valid to
18.07.2029 1. Hans Laukien
2. Isolpack
3. Maas Profilzentrum
4. Montana Bausysteme
5. Wurzer Profiliertechnik
6. Zambelli RIB-ROOF
These companies are representative for the European production of
aluminium profiled sheets.
Additionally, the EPD includes a public annex. This annex applies to:
• 1 m² aluminium sinusoidal profile 18/76
Dipl.-Ing. Hans Peters • 1 kg aluminium profile.
(Chairman of Institut Bauen und Umwelt e.V.) The owner of the declaration shall be liable for the underlying information
and evidence; the IBU shall not be liable with respect to manufacturer
information, life cycle assessment data and evidences.
The EPD was created according to the specifications of EN 15804+A2. In
the following, the standard will be simplified as EN 15804.
Verification
The standard EN 15804 serves as the core PCR
Independent verification of the declaration and data according to ISO
14025:2011
internally X externally
Florian Pronold Mr Olivier Muller,
(Managing Director Institut Bauen und Umwelt e.V.) (Independent verifier)
1 Environmental Product Declaration - PPA-Europe - Profiled sheets made of aluminium for roof, wall and ceiling constructions
Product
Constructional data
Product description/Product definition
1 m² Aluminium trapezoidal profile 35/207
The EPD is valid for prefabricated thin-walled profiled sheets
made of aluminium for loadbearing, self-supporting and non- Name Value Unit
supporting applications in single- and multi-layer roof, wall and Thickness of the sheet, according EN 485-4 0.7 mm
ceiling structures. Surface weight 2.3 kg/m²
Height of the profile, according EN 508 or EN
The profiled sheets are made of a core of aluminium with 35 mm
1090
organic coatings. For the placing of the product on the market
in the European Union / European Free Trade Association Performance data of the product in accordance with the
(EU/EFTA) (with the exception of Switzerland), CPR applies. declaration of performance with respect to its essential
The product needs a Declaration of Performance taking into characteristics according to EN 14782 or EN 1090.
consideration EN 14782 or EN 1090 and the CE-marking. The
Base materials/Ancillary materials
data listed in the respective Declaration of Performance apply.
Aluminium according to EN 485-2 or EN 573-3
For the application and use, the respective national provisions
apply. Organic coating according to EN 12944-1:
Polyester (SP), coil coating, 25 μm on the application side and
Application max. 12 μm on the backside.
The products are used as covering components in single- and
multi-layer roof and wall structures, as well as supporting trays The product does not contain any SVHCs (Substances of Very
in single- and multi-layer roof and ceiling structures for mainly High Concern) REACH.
static loads.
Reference service life
The profiled sheets are used in interior and exterior The term of protection depends on the location, weather
applications. conditions and the quality of the coating, if applicable.
Technical Data Thin-walled profiled sheets made of aluminium exhibit an
Technical specifications for profiled sheets are: estimated service life of > 50 years. This declaration depends
on Life Cycle Assessment and relies on the use conditions,
• EN 14782
according to the BBSR table.
• EN 508
• EN 1090
LCA: Calculation rules
Module C1: Dismantling by the use of machineries- electricity
Declared Unit and diesel driven.
The declared unit is 1 m2 of aluminium profile. The averaging is Module C2: Transport to the site of end-of-life treatment- fixed
done weighted based on the production volume (in m²) per transport distance of 50 km.
company. Module C3: Metal recycling of the aluminium profiles.
Module C4: Deposition/landfill (No environmental impact).
Declared unit
Name Value Unit
Module D: Potential credits for substitution processes or
Declared unit 1 m2 recycling materials from A5 and C3. For the end of life, it is
Surface weight 2.3 kg/m² assumed that the aluminium is recycled with credit for the
Conversion factor to 1 kg 0.44 - recycling potential declared in module D.
For the end of life, a collection rate of 100 % is assumed.
System boundary
Geographic Representativeness
Type of the EPD: cradle to gate - with options, modules C1-C4
Land or region, in which the declared product system is
and module D (A1-A3, C, D and additional modules A4 and A5)
manufactured, used or handled at the end of the product´s
lifespan: Europe
Production stage (modules A1-A3) includes processes that
provide materials and energy input for the system,
manufacturing and transport processes up to the factory gate, Comparability
as well as waste processing. Basically, a comparison or an evaluation of EPD data is only
Module A4: Delivery to the construction site- fixed transport possible if all the data sets to be compared were created
distance of 100 km. according to EN 15804 and the building context, respectively
Module A5: Disposal of transport packaging at the construction the product-specific characteristics of performance, are taken
site and installation by the use of construction machineries - into account. The background datasets are obtained from LCA
electricity and diesel driven. FE (fka GaBi) Database CUP 2023.1.
LCA: Scenarios and additional technical information
Information on describing the biogenic Carbon Content at
Characteristic product properties of biogenic carbon
factory gate
2 Environmental Product Declaration - PPA-Europe - Profiled sheets made of aluminium for roof, wall and ceiling constructions
Name ValueUnit Packaging materials:
PE film 0.06 kg/m² profile
kg
Biogenic carbon content in product - Wooden pallets 0.09 kg/m² profile
C
A5 covers the waste treatment of packaging material at the
Biogenic carbon content in accompanying kg
0.036 point of installation.
packaging C
Name ValueUnit
Note: 1 kg of biogenic carbon is equivalent to 44/12 kg of CO
2 Output substances following waste treatment on
0.152 kg
site
Note: 1 kg of biogenic carbon is equivalent to 44/12 kg of CO .
2 Machine- Diesel driven for installation per kg 0.004 L
Machine- electricity driven for installation per kg 1.89 Wh
The following technical information is a basis for the declared
End of life (C1-C4)
modules.
Name Value Unit
Transport to the building site (A4)
Machine- Diesel driven for installation per kg 0.005 L
Machine- Electricity driven for installation per kg 0.63 Wh
Collected separately waste type waste type 2.3 kg
Name Value Unit
Recycling 2.3 kg
Transport distance 100 km
Landfilling - kg
Capacity utilisation (including empty runs) 61 %
Reuse, recovery or recycling potential (D)
Installation into the building (A5) The avoided production of primary aluminium sheet is
considered. Resulting potential benefits and loads for the metal
recycling are declared in module D.
3 Environmental Product Declaration - PPA-Europe - Profiled sheets made of aluminium for roof, wall and ceiling constructions
LCA: Results
DESCRIPTION OF THE SYSTEM BOUNDARY (X = INCLUDED IN LCA; MND = MODULE OR INDICATOR NOT DECLARED; MNR
= MODULE NOT RELEVANT)
Benefits and
Construction loads beyond
Product stage Use stage End of life stage
process stage the system
boundaries
la ire ta m w a Ry lp p u s tro p s n a rT g n iru tc a fu n a M e h t m o rf tro p s n a rTe tis e h t o t e ta g y lb m e s s A e s U e c n a n e tn ia M ria p e R tn e m e c a lp e R tn e m h s ib ru fe R y g re n e la n o ita re p Oe s u re ta w la n o ita re p Oe s u n o itc u rts n o c -e Dn o itilo m e d tro p s n a rT g n is s e c o rp e ts a W la s o p s iD -e s u e R-y re v o c e R-g n ilc y c e Rla itn e to p
A1 A2 A3 A4 A5 B1 B2 B3 B4 B5 B6 B7 C1 C2 C3 C4 D
X X X X X MND MND MNR MNR MNR MND MND X X X X X
RESULTS OF THE LCA - ENVIRONMENTAL IMPACT according to EN 15804+A2: 1 m² Aluminium trapezoidal profile 35/207
(2.3kg/m²)
Parameter Unit A1-A3 A4 A5 C1 C2 C3 C4 D
GWP-total kg CO 2 eq 2.11E+01 1.67E-02 3.69E-01 1.07E-01 8.35E-03 0 0 -1.96E+01
GWP-fossil kg CO 2 eq 2.12E+01 1.65E-02 2.36E-01 1.05E-01 8.25E-03 0 0 -1.95E+01
GWP-biogenic kg CO 2 eq -1.32E-01 4.87E-05 1.32E-01 4.18E-04 2.44E-05 0 0 -3.85E-02
GWP-luluc kg CO 2 eq 5.74E-03 1.53E-04 8.21E-04 9.69E-04 7.64E-05 0 0 -1.77E-03
ODP kg CFC11 eq 2.28E-11 2.15E-15 1.37E-10 2.12E-14 1.07E-15 0 0 -1.62E-11
AP mol H+ eq 9.75E-02 2.12E-05 5.79E-04 6.15E-04 1.06E-05 0 0 -6.8E-02
EP-freshwater kg P eq 1.24E-05 6.04E-08 3.33E-07 3.84E-07 3.02E-08 0 0 -6.54E-06
EP-marine kg N eq 1.45E-02 7.18E-06 2.73E-04 3E-04 3.59E-06 0 0 -1.16E-02
EP-terrestrial mol N eq 1.58E-01 8.64E-05 3.07E-03 3.32E-03 4.32E-05 0 0 -1.26E-01
kg NMVOC
POCP 4.43E-02 1.83E-05 7.25E-04 7.98E-04 9.13E-06 0 0 -3.43E-02
eq
ADPE kg Sb eq 1.1E-06 1.09E-09 6.15E-09 6.96E-09 5.44E-10 0 0 -6.81E-07
ADPF MJ 2.85E+02 2.25E-01 1.3E+00 1.43E+00 1.12E-01 0 0 -2.63E+02
m3 world eq
WDP 3.1E+00 1.99E-04 3.09E-02 1.36E-03 9.97E-05 0 0 -1.2E+00
deprived
GWP = Global warming potential; ODP = Depletion potential of the stratospheric ozone layer; AP = Acidification potential of land and water; EP =
Eutrophication potential; POCP = Formation potential of tropospheric ozone photochemical oxidants; ADPE = Abiotic depletion potential for non-fossil
resources; ADPF = Abiotic depletion potential for fossil resources; WDP = Water (user) deprivation potential)
RESULTS OF THE LCA - INDICATORS TO DESCRIBE RESOURCE USE according to EN 15804+A2: 1 m² Aluminium trapezoidal
profile 35/207 (2.3kg/m²)
Parameter Unit A1-A3 A4 A5 C1 C2 C3 C4 D
PERE MJ 1.22E+02 1.64E-02 1.7E+00 1.09E-01 8.18E-03 0 0 -8.64E+01
PERM MJ 1.58E+00 0 -1.58E+00 0 0 0 0 0
PERT MJ 1.24E+02 1.64E-02 1.1E-01 1.09E-01 8.18E-03 0 0 -8.64E+01
PENRE MJ 2.83E+02 2.26E-01 4.13E+00 1.44E+00 1.13E-01 0 0 -2.64E+02
PENRM MJ 2.83E+00 0 -2.83E+00 0 0 0 0 0
PENRT MJ 2.85E+02 2.26E-01 1.31E+00 1.44E+00 1.13E-01 0 0 -2.64E+02
SM kg 0 0 0 0 0 0 0 0
RSF MJ 2.65E-22 0 0 0 0 0 0 0
NRSF MJ 3.11E-21 0 0 0 0 0 0 0
FW m3 2.95E-01 1.79E-05 8.01E-04 1.18E-04 8.96E-06 0 0 -1.8E-01
PERE = Use of renewable primary energy excluding renewable primary energy resources used as raw materials; PERM = Use of renewable primary
energy resources used as raw materials; PERT = Total use of renewable primary energy resources; PENRE = Use of non-renewable primary energy
excluding non-renewable primary energy resources used as raw materials; PENRM = Use of non-renewable primary energy resources used as raw
materials; PENRT = Total use of non-renewable primary energy resources; SM = Use of secondary material; RSF = Use of renewable secondary fuels;
NRSF = Use of non-renewable secondary fuels; FW = Use of net fresh water
RESULTS OF THE LCA – WASTE CATEGORIES AND OUTPUT FLOWS according to EN 15804+A2:
1 m² Aluminium trapezoidal profile 35/207 (2.3kg/m²)
Parameter Unit A1-A3 A4 A5 C1 C2 C3 C4 D
HWD kg 1.91E-08 6.99E-13 2.47E-12 3.75E-12 3.49E-13 0 0 2.89E-08
NHWD kg 5.9E+00 3.44E-05 2.84E-03 2.25E-04 1.72E-05 0 0 -4.48E+00
RWD kg 1.65E-02 4.22E-07 1.03E-05 4.06E-06 2.11E-07 0 0 -2.03E-02
CRU kg 0 0 0 0 0 0 0 0
MFR kg 7.62E-02 0 0 0 0 2.3E+00 0 0
MER kg 0 0 0 0 0 0 0 0
EEE MJ 0 0 4.15E-01 0 0 0 0 0
EET MJ 0 0 1.07E+00 0 0 0 0 0
4 Environmental Product Declaration - PPA-Europe - Profiled sheets made of aluminium for roof, wall and ceiling constructions
HWD = Hazardous waste disposed; NHWD = Non-hazardous waste disposed; RWD = Radioactive waste disposed; CRU = Components for re-use;
MFR = Materials for recycling; MER = Materials for energy recovery; EEE = Exported electrical energy; EET = Exported thermal energy
RESULTS OF THE LCA – additional impact categories according to EN 15804+A2-optional:
1 m² Aluminium trapezoidal profile 35/207 (2.3kg/m²)
Parameter Unit A1-A3 A4 A5 C1 C2 C3 C4 D
Disease
PM 1.1E-06 1.55E-10 1.06E-08 1.22E-08 7.75E-11 0 0 -7.24E-07
incidence
IR kBq U235 eq 3.34E+00 6.3E-05 1.36E-03 6.29E-04 3.15E-05 0 0 -4.49E+00
ETP-fw CTUe 9.75E+01 1.6E-01 9.18E-01 1.02E+00 7.99E-02 0 0 -9.54E+01
HTP-c CTUh 1.19E-08 3.27E-12 2.02E-11 2.08E-11 1.63E-12 0 0 -8.14E-09
HTP-nc CTUh 2.48E-07 1.74E-10 1.32E-09 1.37E-09 8.7E-11 0 0 -1.92E-07
SQP SQP 4.18E+01 9.4E-02 5.25E-01 5.99E-01 4.7E-02 0 0 -7.26E+00
PM = Potential incidence of disease due to PM emissions; IR = Potential Human exposure efficiency relative to U235; ETP-fw = Potential comparative
Toxic Unit for ecosystems; HTP-c = Potential comparative Toxic Unit for humans (cancerogenic); HTP-nc = Potential comparative Toxic Unit for humans
(not cancerogenic); SQP = Potential soil quality index
Disclaimer 1 – concerning Potential Human exposure efficiency relative to U235 (IRP) - This impact category deals mainly with the
eventual impact of low-dose ionizing radiation on human health of the nuclear fuel cycle. It does not consider effects due to possible
nuclear accidents, occupational exposure or radioactive waste disposal in underground facilities. Potential ionizing radiation from the
soil, radon and from some construction materials is also not measured by this indicator.
Disclaimer 2 – concerning (ADP-minerals & metals, ADP-fossil, WDP, ETP-fwm HTP-c, HTP-nc, SQP) - The results of this
environmental impact indicator shall be used with care as the uncertainties on these results are high as there is limited experience with
the indicator.
References
EN 485-2 http://www.nachhaltigesbauen.de/baustoff-und-
Aluminium and aluminium alloys - Sheet, strip and plate - Part gebaeudedaten/nutzungsdauern-von-bauteilen.html
2: Mechanical properties
CPR
EN 508-2 REGULATION (EU) No 305/2011 OF THE EUROPEAN
Roofing products from metal sheet - Specification for self- PARLIAMENT AND OF THE COUNCIL of 9 March 2011 laying
supporting products of steel, aluminium or stainless steel down harmonised conditions for the marketing of construction
sheet - Part 2: Aluminium products and repealing Council Directive 89/106/EEC
EN 573-3 IBU PCR Part A
Aluminium and aluminium alloys - Chemical composition and PCR - Part A: Calculation rules for the Life Cycle Assessment
form of wrought products - Part 3: Chemical composition and and Requirements on the Background Report, version 1.3,
form of products Institut Bauen und Umwelt e.V., www.bau-umwelt.com, August
2021
EN 1090-1
Execution of steel structures and aluminium structures - Part 1: IBU PCR Part B
Requirements for conformity assessment of structural PCR – Part B: Requirements of the EPD for Thin walled profiles
components and profiled panels of metal, v8, Institut Bauen und Umwelt
e.V., www.bau-umwelt.com, 2023-10
EN 1090-5
Execution of steel structures and aluminium structures - Part 5: LCA FE Software and Database
Technical requirements for cold-formed structural aluminium LCA FE software-system and CUP 2023.1 databases,
elements and cold-formed structures for roof, ceiling, floor and University of Stuttgart and Sphera Solutions GmbH,
wall applications LeinfeldenEchterdingen, 2023 (https://sphera.com/product-
sustainabilitygabi-data-search/)
EN ISO 12944-1
Paints and varnishes - Corrosion protection of steel structures
by protective coating systems - Part 1: General introduction
EN 14782
Self-supporting metal sheet for roofing, external cladding and
internal lining - Product specification and requirements
EN 15804+ A2: 2019
Sustainability of construction works -Environmental Product
Declarations - Core rules for the product category of
construction products
BBSR table
BBSR table (german):
'Nutzungsdauern von Bauteilen zur Lebenszyklusanalyse nach
BNB', Federal Institute for Research on Building, Urban Affairs
and Spatial Development, Referat II Nachhaltiges Bauen;
online available under
5 Environmental Product Declaration - PPA-Europe - Profiled sheets made of aluminium for roof, wall and ceiling constructions
6 Environmental Product Declaration - PPA-Europe - Profiled sheets made of aluminium for roof, wall and ceiling constructions
Publisher
Institut Bauen und Umwelt e.V. +49 (0)30 3087748- 0
Hegelplatz 1 info@ibu-epd.com
10117 Berlin www.ibu-epd.com
Germany
Programme holder
Institut Bauen und Umwelt e.V. +49 (0)30 3087748- 0
Hegelplatz 1 info@ibu-epd.com
10117 Berlin www.ibu-epd.com
Germany
Author of the Life Cycle Assessment
Sphera Solutions GmbH +49 (0)711 341817-0
Hauptstraße 111- 113 info@sphera.com
70771 Leinfelden-Echterdingen www.sphera.com
Germany
Owner of the Declaration
European Association for Panels and Profiles e. V. +49 2151 93630-0
(PPA-Europe) info@ppa-europe.eu
Europark Fichtenhain A 13a www.ppa-europe.eu
47807 Krefeld
Germany
7 Environmental Product Declaration - PPA-Europe - Profiled sheets made of aluminium for roof, wall and ceiling constructions
