ENVIRONMENTAL PRODUCT DECLARATION
as per ISO 14025 and EN 15804+A2
Owner of the Declaration Hammerer Aluminium Industries Santana S.R.L.
Publisher Institut Bauen und Umwelt e.V. (IBU)
Programme holder Institut Bauen und Umwelt e.V. (IBU)
Declaration number EPD-HAA-20230201-IBA1-EN
Issue date 15.09.2023
Valid to 14.09.2028
Aluminium billets
Hammerer Aluminium Industries Santana S.R.L.
www.ibu-epd.com | https://epd-online.com
1. General Information
Hammerer Aluminium Industries Santana Aluminium billets
S.R.L.
Programme holder Owner of the declaration
IBU – Institut Bauen und Umwelt e.V. Hammerer Aluminium Industries Santana S.R.L.
Hegelplatz 1 Calea Hammerer 5
10117 Berlin 317280 Santana
Germany Romania
Declaration number Declared product / declared unit
EPD-HAA-20230201-IBA1-EN The declared product is 1 kg of aluminium billets.
This declaration is based on the product category rules: Scope:
Products of aluminium and aluminium alloys, 01.08.2021 This product declaration refers to a declared unit of 1 kg of aluminium
(PCR checked and approved by the SVR) billets produced in one production facility in Sântana, Romania.
The owner of the declaration shall be liable for the underlying information
and evidence; the IBU shall not be liable with respect to manufacturer
Issue date information, life cycle assessment data and evidences.
15.09.2023
The EPD was created according to the specifications of EN 15804+A2. In
the following, the standard will be simplified as EN 15804.
Valid to
Verification
14.09.2028
The standard EN 15804 serves as the core PCR
Independent verification of the declaration and data according to ISO
14025:2011
internally X externally
Dipl.-Ing. Hans Peters
(Chairman of Institut Bauen und Umwelt e.V.)
Florian Pronold Dr. Eva Schmincke,
(Managing Director Institut Bauen und Umwelt e.V.) (Independent verifier)
1 Environmental-Product Declaration - Hammerer Aluminium Industries Santana S.R.L. - Aluminium billets
2. Product
Concern (SVHC) above 0.1 mass %.
2.1 Product description/Product definition
This EPD refers to 1 kg of aluminium billets consisting of The product/at least one sub-product does not contain other
primary and recycled aluminium, reinforced by alloying carcinogenic, mutagenic, reprotoxic (CMR) substances of
elements. category 1A or 1B not on the candidate list above 0.1 mass %
For the use and application of the product, the respective in at least one sub-product.
national provisions at the place of use apply.
2.2 Application
No biocidal products have been added to the present
The final aluminium product (aluminium billets) is used for construction product or it has been treated with biocidal
creating different aluminium products, for industry, building and products (it is thus a treated product within the meaning of the
construction, and automotive industries. Biocidal Products Regulation (EU) No 528/2012).
2.3 Technical Data 2.6 Manufacture
The physical properties correspond to aluminium billets The main technological flow in Hammerer Aluminium Industries
products. The chemical composition of the aluminium billets is is the development of secondary aluminium by recycling
based on the EN AW-6060 specifications. aluminium waste in melting furnaces. The casting activity is
carried out in several stages, as follows:
The final product has the characteristics described in the table
below.
Constructional data
Name Value Unit
Gross density 2700 kg/m3
Melting point 650 °C
Electrical conductivity at 20°C - m/Ωmm2
Thermal conductivity 220 W/(mK)
Coefficient of thermal expansion 23.4 10-6K-1
Modulus of elasticity 69500 N/mm2
Shear modulus 26100 N/mm2
Specific heat capacity 0.898 kJ/kgK
Hardness 75 HB
Yield strength Rp 0,2 min. 160 N/mm2
Tensile strength Rm min. 215 N/mm2
Tensile stress at break 14 %
Note that the values for Hardness, Yield strength Rp 0,2 min., There are two production lines: Line 1, where aluminium waste
Tensile strength Rm min. and Tensile stress at break, are the with high aluminium quantities is melted and casted in semi-
maximum ones. The mechanical properties after extrusion and finished products and Line 2, where aluminium waste with lower
heat treatment, depend on temper. aluminium quantities and dross (slag) is melted and casted. In
addition to that, aluminium ingots of primary aluminium are
Performance data of the product with respect to its delivered to the furnaces, where they are heated and mixed
characteristics in accordance with the relevant technical with secondary aluminium, originating from pre- and post-
provision (no CE-marking). consumer scrap and aluminium-rich waste from Line 2. The
industrial products made are intended for the Business-to-
2.4 Delivery status business market segment.
The aluminium billets are delivered on the desired length and
diameter. The most common length is 7 meters. The billets are The company has implemented a certified quality management
secured during transport by being tied together using plastic system, IATF 16949, which monitors the entire manufacturing
bands and placed on rectangular wooden bars. process.
2.5 Base materials/Ancillary materials 2.7 Environment and health during manufacturing
The main constituent of the aluminium billets is aluminium with The production facility has an environmental management
a share of around 99% and alloying metals in a percentage of system in accordance with ISO 14001, an energy management
around 1 %. in accordance with ISO 50001 and an occupational health and
safety management system in accordance with ISO 45001 in
The share of aluminium in the product consists of about 21 % order to ensure environmental protection and occupational
primary aluminium and around 78 % of recycled aluminium and health and safety in the production process.
scrap.
From the total amount of primary aluminium, HAI purchases 2.8 Product processing/Installation
around 71 % of it from a supplier that provides a low carbon The aluminium billets are delivered to different industries and
aluminium. the processing/installation depends on each individual industry.
Some of the processing activities of aluminium billets are, but
The product/at least part of the product does not contain not limited to extrusion and forging.
substances on the ECHA list of Substances of Very High
2.9 Packaging
2 Environmental-Product Declaration - Hammerer Aluminium Industries Santana S.R.L. - Aluminium billets
The billets are tied together with plastic straps and placed on class A "non-combustible" according to DIN 4102-4.The melting
rectangular wooden bars. The number of billets tied together point of aluminium is approx. 650° C.
and the length may differ, based on customers' requests. The toxicity of fire gases is not applicable.
Fire protection
Both the wooden bars and the plastic straps can be recycled by
Name Value
the customer.
Building material class A1
2.10 Condition of use Burning droplets Not applicable
The aluminium billets are produced based on EN AW-6060
Smoke gas development Not applicable
specifications.
There are no special features of the material composition for
the period of use. Water
The exposure of the aluminium billets to water does not alter
2.11 Environment and health during use the product and has no negative impact on the environment
If the aluminium billets are used as intended, no hazards to air, (water).
water and soil as well as to human health can arise.
Mechanical destruction
No harmful substances are incorporated in the product. Unforeseen mechanical destruction of the aluminium billets is
not relevant.
The environmental impact during the use phase depends on
2.14 Re-use phase
the design of the end product since aluminium billets are not
finished products. The aluminium billets are 100 % recyclable. The material does
not suffer any loss of quality and can be recycled forever. The
2.12 Reference service life scrap resulting in the production process is processed into new
The aluminium billets are not a final product and they are used aluminium billets.
for different industries as input material where it can have The aluminium scrap from demolition can be separated,
multiple applications, therefore no reference service life (RSL) collected and recycled by the recycling industry.
is declared for aluminium billets.
2.15 Disposal
The aluminium billets are not a finished product and they are
used as inputs for different industries. Each industry might treat According to the European Waste Catalog (EWC), the disposal
the aluminium based on the properties of the environment code depends on the end product.
where the finished products will stand. The treatment will Given its high value, the aluminium scrap it's not disposed but
influence the ageing of the final product. used as a raw material in the recycling industry.
2.13 Extraordinary effects 2.16 Further information
Fire For more information, visit: https://www.hai-aluminium.com/
Aluminium billets meet the requirements of building material
3. LCA: Calculation rules
national grid.
3.1 Declared Unit • The electricity is 100 % green electricity based on the
The declared unit refers to 1 kg of aluminium billets, from a contract concluded between HAI and the electricity
single major production line (Remelting and Casting). The supplier.
product consists of primary and recycled aluminium (99 %), Module C2 | Transport to waste processing
reinforced by alloying elements (~1 %). There are no by- Module C2 declares the environmental impacts resulting from
products formed from the production line subject to this study. transporting the waste aluminium to a waste processing facility
Declared unit and mass reference at an assumed distance of 50 km.
Name Value Unit
Module C3 | Waste processing
Declared unit 1 kg
Module C3 declares the environmental impacts resulting from
the treatment of aluminium scrap by collecting, sorting, cleaning
Data used in calculations represent site-specific production and pressing (90 % of the product).
volumes for 2022 of the main product line.
Module C4 | Disposal
3.2 System boundary Module C4 declares the environmental impacts resulting from
The LCA for aluminium billets is a cradle-to-gate assessment of landfilling (10 % of the product).
the environmental impacts with options.
The following life cycle phases are considered in the analysis: Module D | Credits and loads outside the system boundary
Module A1-A3 | Product stage In Module D, the substitution potential of primary aluminium
The following processes were considered: through a recycling scenario (90 % of the product) is presented.
• The purchase of the raw materials and the ancillary
3.3 Estimates and assumptions
materials such as primary aluminium, recycled
This study analysis is based mainly on on-site specific data
aluminium as well as ancillary materials such as alloying
related to product manufacturing. Study results are valid for the
metals and packaging.
technological process specified, geographical area and time
• The transport of the raw and ancillary materials was
period mentioned.
calculated based on the actual distances of the
Furthermore, the following estimates have been made:
suppliers.
• The energy consists of diesel used in the manufacturing • Alloys – for the purpose of calculations all alloys are
process and natural gas which is supplied from the assumed to
3 Environmental-Product Declaration - Hammerer Aluminium Industries Santana S.R.L. - Aluminium billets
be pure substances, thus containing 100 % of a given
substance (e.g. Mg, Zn). The alloys contribute about 1 3.5 Background data
% to the final product. Calculations were performed using Simapro 9.4.0.2, where
• Starting with 2021, HAI is purchasing only green inputs and outputs are listed. The LCA impacts were calculated
electricity. The actual energy mix will be published after using characterization factors from Ecoinvent 3.8 database,
this study was performed. A 75 % hydro-power and 25 applying the EN 15804 + A2 Method V1.03 / EF 3.0
% wind power was assumed as electricity mix. normalization and weighting set.
• It was assumed that soft sawn wood with a density of
3.6 Data quality
540 kg/m3 is used for wood packaging.
Data reliability is ensured by the manufacturer's data
• The use of Euro 6 trucks is assumed for the transport,
management systems and expert knowledge of plant
due to the prevalence of this type of Euro trucks in the
engineers. Additional questions regarding reported values (e.g.,
fleet transporting materials.
type of material, materials use, waste management techniques,
• For all inputs a dataset representative for the European
transportation distances, etc.) were answered and clarified by
market was selected (if available) or a global market
plant engineers.
dataset in case a European dataset was not available.
• Only the environmental burden from collection, sorting
3.7 Period under review
and transportation of Al scrap used as an input is
Site-specific data is collected for all flows according to the set
accounted for.
cut-off criteria. Data collected is representative of one and the
• All waste outputs such as mixed plastic, wood,
same technology for the period between the 1st of January
cardboard, are accounted for by selecting datasets
2022 to the 31st of December 2022. All the collected data is
representative for the market, where transport is already
based on the actual quantities used and produced during this
included in the final assessment of the impacts.
period.
Respective types of waste treatment have been
selected (preparation for recycling, incineration,
3.8 Geographic Representativeness
landfilling).
Land or region, in which the declared product system is
• The amount of used water is accounted as tap water
manufactured, used or handled at the end of the product´s
from municipal supply or underground water without
lifespan: Europe
treatment depending on the reported quantities.
• In 2022 part of the production of the same line was a
specific different product (specific customer 3.9 Allocation
requirement). The technological process is identical to
In this study there are no by-products and thus no relevant
the studied product, the only difference being the share
allocation is considered necessary since all inputs are
of alloys, especially the share of magnesium in its
converted to the main product described above and waste
content. As this product is not representative for the
outflows.
studied product, the quantity of magnesium used in this
The total environmental burden is associated with the products
study was adjusted to reflect the production of the
delivered to the customers
studied product. The production process is identical and
no other inputs needed adjustments. 3.10 Comparability
Basically, a comparison or an evaluation of EPD data is only
3.4 Cut-off criteria possible if all the data sets to be compared were created
All inputs and outputs from background system to foreground according to EN 15804 and the building context, respectively
system processes, with significant potential impact, are the product-specific characteristics of performance, are taken
included in the calculation, as company specific data is into account.
available. Cut-off criteria are set to be not more than 1% of Calculations were performed using Simapro 9.4.0.2, where
renewable and non-renewable primary energy usage and not inputs and outputs are listed. The LCA impacts were calculated
more than 1% of the total mass flow for a single flow and 99% using characterization factors from Ecoinvent 3.8 database.
of all flows are considered.
4. LCA: Scenarios and additional technical information
Association.
Characteristic product properties biogenic carbon
Name Value Unit
Biogenic carbon is present only in the wooden packaging and it
Recycling 0.9 kg
is not reported since the wood packaging represents less than
1 % from the total inputs of packaging. Landfilling 0.1 kg
Reuse, recovery and/or recycling potentials (D), relevant
End of life (C1-C4) scenario information
For the end-of-life scenario used in this study the following
Name Value Unit
assumptions and thus follows the most recent data on
Recycling 90 %
aluminium recycling published by the European Aluminium
4 Environmental-Product Declaration - Hammerer Aluminium Industries Santana S.R.L. - Aluminium billets
5. LCA: Results
The following table shows the LCA results for the declared unit of 1 kg of aluminium billets.
DESCRIPTION OF THE SYSTEM BOUNDARY (X = INCLUDED IN LCA; ND = MODULE OR INDICATOR NOT DECLARED; MNR =
MODULE NOT RELEVANT)
Benefits and
Construction loads beyond
Product stage Use stage End of life stage
process stage the system
boundaries
la ire ta m w a Ry lp p u s tro p s n a rT g n iru tc a fu n a M e h t m o rf tro p s n a rTe tis e h t o t e ta g y lb m e s s A e s U e c n a n e tn ia M ria p e R tn e m e c a lp e R tn e m h s ib ru fe R y g re n e la n o ita re p Oe s u re ta w la n o ita re p Oe s u n o itc u rts n o c -e Dn o itilo m e d tro p s n a rT g n is s e c o rp e ts a W la s o p s iD -e s u e R-y re v o c e R-g n ilc y c e Rla itn e to p
A1 A2 A3 A4 A5 B1 B2 B3 B4 B5 B6 B7 C1 C2 C3 C4 D
X X X MND MND MND MND MNR MNR MNR MND MND MND X X X X
RESULTS OF THE LCA - ENVIRONMENTAL IMPACT according to EN 15804+A2: 1 kg aluminium billets
Parameter Unit A1-A3 C2 C3 C4 D
Global Warming Potential total (GWP-total) kg CO 2 eq 1.93E+00 1.07E-02 2.4E-01 5.56E-03 -1.74E+00
Global Warming Potential fossil fuels (GWP-fossil) kg CO 2 eq 1.88E+00 1.07E-02 2.38E-01 5.52E-03 -1.7E+00
Global Warming Potential biogenic (GWP-biogenic) kg CO 2 eq 3.32E-03 1.03E-05 1.72E-03 3.92E-05 -5.82E-03
Global Warming Potential luluc (GWP-luluc) kg CO 2 eq 3.95E-02 5.04E-06 3.2E-04 5.09E-06 -3.33E-02
Depletion potential of the stratospheric ozone layer (ODP) kg CFC11 eq 1.41E-07 2.41E-09 1.11E-08 7.62E-10 -1.2E-07
Acidification potential of land and water (AP) mol H+ eq 2E-02 3.02E-05 9.57E-04 3.4E-05 -1.31E-02
Eutrophication potential aquatic freshwater (EP-freshwater) kg P eq 1.96E-04 8.05E-07 6.74E-05 1.3E-06 -7.74E-04
Eutrophication potential aquatic marine (EP-marine) kg N eq 3.88E-03 5.9E-06 1.35E-04 9.08E-06 -1.72E-03
Eutrophication potential terrestrial (EP-terrestrial) mol N eq 2.18E-02 6.42E-05 1.49E-03 9.81E-05 -1.71E-02
kg NMVOC
Formation potential of tropospheric ozone photochemical oxidants (POCP) 6.93E-03 2.46E-05 4.28E-04 2.93E-05 -5.71E-03
eq
Abiotic depletion potential for non fossil resources (ADPE) kg Sb eq 5.85E-06 4.88E-08 1.1E-05 1.39E-08 1.42E-05
Abiotic depletion potential for fossil resources (ADPF) MJ 2.72E+01 1.6E-01 1.56E+00 7.88E-02 -2.14E+01
m3 world eq
Water use (WDP) 4.24E-01 5.3E-04 2.02E-02 1.53E-03 -2.71E-01
deprived
RESULTS OF THE LCA - INDICATORS TO DESCRIBE RESOURCE USE according to EN 15804+A2: 1 kg aluminium billets
Parameter Unit A1-A3 C2 C3 C4 D
Renewable primary energy as energy carrier (PERE) MJ 1.33E+01 2.7E-03 2.09E-01 4.05E-03 -8.16E+00
Renewable primary energy resources as material utilization (PERM) MJ 7.74E-03 0 0 0 0
Total use of renewable primary energy resources (PERT) MJ 1.33E+01 2.7E-03 2.09E-01 4.05E-03 -8.16E+00
Non renewable primary energy as energy carrier (PENRE) MJ 2.72E+01 1.6E-01 1.57E+00 7.88E-02 -2.14E+01
Non renewable primary energy as material utilization (PENRM) MJ 0 0 0 0 0
Total use of non renewable primary energy resources (PENRT) MJ 2.72E+01 1.6E-01 1.57E+00 7.88E-02 -2.14E+01
Use of secondary material (SM) kg 7.88E-01 0 0 0 0
Use of renewable secondary fuels (RSF) MJ 0 0 0 0 0
Use of non renewable secondary fuels (NRSF) MJ 0 0 0 0 0
Use of net fresh water (FW) m3 2.29E-03 0 0 0 0
RESULTS OF THE LCA – WASTE CATEGORIES AND OUTPUT FLOWS according to EN 15804+A2:
1 kg aluminium billets
Parameter Unit A1-A3 C2 C3 C4 D
Hazardous waste disposed (HWD) kg 3.17E-05 4.28E-07 5.94E-03 1.15E-07 2.41E-04
Non hazardous waste disposed (NHWD) kg 7.48E-01 6.79E-03 1.38E-01 2.06E-01 -4.71E-01
Radioactive waste disposed (RWD) kg 1.66E-04 1.07E-06 6.49E-06 3.72E-07 -8.64E-05
Components for re-use (CRU) kg 0 0 0 0 0
Materials for recycling (MFR) kg 1.22E-03 0 0 0 0
Materials for energy recovery (MER) kg 0 0 0 0 0
Exported electrical energy (EEE) MJ 0 0 0 0 0
Exported thermal energy (EET) MJ 0 0 0 0 0
RESULTS OF THE LCA – additional impact categories according to EN 15804+A2-optional:
1 kg aluminium billets
Parameter Unit A1-A3 C2 C3 C4 D
Disease
Incidence of disease due to PM emissions (PM) 2.87E-07 7.29E-10 1.47E-08 5.86E-10 -1.39E-07
incidence
Human exposure efficiency relative to U235 (IR) kBq U235 eq 4.33E-01 8.49E-04 1.61E-02 4.5E-04 -2.35E-01
Comparative toxic unit for ecosystems (ETP-fw) CTUe 5.83E+01 4.61E-02 5.68E-01 1.58E-01 -2.1E+01
Comparative toxic unit for humans (carcinogenic) (HTP-c) CTUh 9.35E-09 2.18E-12 5.04E-11 2.82E-12 -4.48E-09
Comparative toxic unit for humans (noncarcinogenic) (HTP-nc) CTUh 8.61E-08 1.26E-10 6.93E-09 1.14E-10 -6.3E-08
5 Environmental-Product Declaration - Hammerer Aluminium Industries Santana S.R.L. - Aluminium billets
Soil quality index (SQP) SQP 1.15E+01 9.45E-02 1.49E+00 9.88E-02 -1.26E+00
Disclaimer 1 – for the indicator “Potential Human exposure efficiency relative to U235”. This impact category deals mainly with the
eventual impact of low-dose ionizing radiation on human health of the nuclear fuel cycle. It does not consider effects due to possible
nuclear accidents, occupational exposure nor due to radioactive waste disposal in underground facilities. Potential ionizing radiation
from the soil, from radon and from some construction materials is also not measured by this indicator.
Disclaimer 2 – for the indicators “abiotic depletion potential for non-fossil resources”, “abiotic depletion potential for fossil resources”,
“water (user) deprivation potential, deprivation-weighted water consumption”, “potential comparative toxic unit for ecosystems”,
“potential comparative toxic unit for humans – cancerogenic”, “Potential comparative toxic unit for humans - not cancerogenic”,
“potential soil quality index”. The results of this environmental impact indicator shall be used with care as the uncertainties on these
results are high or as there is limited experienced with the indicator.
6. LCA: Interpretation
The LCA results are presented for 1 kg of aluminium billets. The
charts below provide information on the impacts per main In the figure below it can be seen that by excluding the final
processes of the upstream and manufacturing life cycle stages. disposal materials still represent the dominant category and are
There are no known limitations to the results in the context of responsible for 82 % of the total climate change impact
the set goal and scope of the study. category.
Based on the results it can be concluded that the dominant
material category appears to be materials responsible for
81.58% for climate change category. The second biggest
contributor to the overall impact is energy with 13.26 % for
climate change category followed by the footprint of the
transportation with a share of 4.74 % for climate change
category.
7. Requisite evidence
The product is not a finished product (end product) and it is application of the final product.
used as raw material for other industries. The processing and
the design of the end product will vary, depending on the
8. References
Standards
ISO 14040
DIN EN 573-3:2019-10 ISO 14040:2006, Environmental management — Life cycle
Aluminium and aluminium alloys - Chemical composition and assessment — Principles and framework
form of wrought products - Part 3: Chemical composition and
form of products ISO 14044
ISO 14044:2006, Environmental management — Life cycle
DIN 4102-4 assessment — Requirements and guidelines
Fire behaviour of building materials and building components -
Part 4: Synopsis and application of classified building materials, EN 15804
components and special components EN 15804:2012+A2:2019+AC:2021, Sustainability of
construction works — Environmental Product Declarations —
IATF 16949 Core rules for the product category of construction products.
IATF 16949:2016 Quality management system for
organizations in the automotive industry ISO 45001
ISO 45001:2018 Occupational health and safety management
ISO 14001 systems
ISO 14001:2015 Environmental management systems
ISO 14025 ISO 50001
EN ISO 14025:2011, Environmental labels and declarations — ISO 50001:2018 Energy management systems
Type III environmental declarations — Principles and Further References
procedures.
6 Environmental-Product Declaration - Hammerer Aluminium Industries Santana S.R.L. - Aluminium billets
BPR Regulation EPD programme of Institut Bauen und Umwelt e.V., Version
Biocidal Products Regulation EU 528/2012 2.0, Berlin: Institut Bauen und Umwelt e.V., 2021, www.ibu-
epd.com
European Aluminium Association
A strategy for achieving aluminium's full potential for circular PCR Part A: Calculation Rules for the Life Cycle Assessment
economy by 2030 and Requirements on the Project Report according to EN
https://european-aluminium.eu/wp- 15804+A2:2019, v. 1.3
content/uploads/2022/08/european-aluminium-circular-
aluminium-action-plan.pdf PCR Part B: Requirements on the EPD for Products of
aluminium and aluminium alloys, v. 1.6
ECHA list
List of substances of very high concern (SVHC) for Software and database
authorisation (ECHA Candidate List), 14.01.2020, published
under Article 59(10) of REACH. Helsinki: European Chemicals SimaPro
Agency. http://echa.europa.eu/ LCA and reporting softwareapps.simapro.com
European Waste Catalogue (EWC)
Ordinance on the European Waste List (Waste List Ordinance ecoinvent Version 3
AVV) Wernet, G., Bauer, C., Steubing, B., Reinhard, J., Moreno-Ruiz,
E., and Weidema, B., 2016. The ecoinvent database version 3
IBU (part I): overview and methodology. The International Journal of
Institut Bauen und Umwelt e.V.: General Instructions for the Life Cycle Assessment, [online] 21(9), pp.1218–1230.
7 Environmental-Product Declaration - Hammerer Aluminium Industries Santana S.R.L. - Aluminium billets
Publisher
Institut Bauen und Umwelt e.V. +49 (0)30 3087748- 0
Hegelplatz 1 info@ibu-epd.com
10117 Berlin www.ibu-epd.com
Germany
Programme holder
Institut Bauen und Umwelt e.V. +49 (0)30 3087748- 0
Hegelplatz 1 info@ibu-epd.com
10117 Berlin www.ibu-epd.com
Germany
Author of the Life Cycle Assessment
denkstatt Bulgaria OOD +359 2 470 7508
Lyubata 4-6 office@denkstatt.bg
1407 Sofia http://denkstatt.bg/
Bulgaria
Owner of the Declaration
Hammerer Aluminium Industries Santana S.R.L. +40 751 078 857
Calea Hammerer 5 Andreia.Godea@hai-
317280 Santana aluminium.com
Romania www.hai-aluminium.com
8 Environmental-Product Declaration - Hammerer Aluminium Industries Santana S.R.L. - Aluminium billets
