ENVIRONMENTAL PRODUCT DECLARATION
as per ISO 14025 and EN 15804+A2
Owner of the Declaration dormakaba International Holding GmbH
Publisher Institut Bauen und Umwelt e.V. (IBU)
Programme holder Institut Bauen und Umwelt e.V. (IBU)
Declaration number EPD-DOR-20230101-CBA4-EN
Issue date 14.04.2023
Valid to 13.04.2028
ARGUS V60
dormakaba
www.ibu-epd.com | https://epd-online.com
General Information
dormakaba ARGUS V60
Programme holder Owner of the declaration
IBU – Institut Bauen und Umwelt e.V. dormakaba International Holding GmbH
Hegelplatz 1 DORMA Platz 1
10117 Berlin 58256 Ennepetal
Germany Germany
Declaration number Declared product / declared unit
EPD-DOR-20230101-CBA4-EN 1 piece of the product: Sensor Barrier ARGUS V60, consisting of the
following items:
- Housings
- Tempered safety glasses (6 mm)
- Cover plates
- Glass door leaves (10 mm)
- Drive unit
- Sensor technology
- LED status display
- Product packaging
This declaration is based on the product category rules: Scope:
Electronic and physical Access Control Systems, 01.08.2021 This Environmental Product Declaration refers to a specific ARGUS V60
(PCR checked and approved by the SVR) sensor barrier manufactured by dormakaba. The production site is located
in Bühl (Germany). Green electricity is being used at this production site.
Issue date Data represents the year 2022.
The owner of the declaration shall be liable for the underlying information
14.04.2023
and evidence; the IBU shall not be liable with respect to manufacturer
information, life cycle assessment data and evidences.
Valid to
The EPD was created according to the specifications of EN 15804+A2. In
13.04.2028 the following, the standard will be simplified as EN 15804.
Verification
The standard EN 15804 serves as the core PCR
Independent verification of the declaration and data according to ISO
14025:2011
internally X externally
Dipl.-Ing. Hans Peters
(Chairman of Institut Bauen und Umwelt e.V.)
Florian Pronold Dr.-Ing. Wolfram Trinius,
(Managing Director Institut Bauen und Umwelt e.V.) (Independent verifier)
1 Environmental Product Declaration - dormakaba - ARGUS V60
Product
ARGUS V60 sensor barriers have the following technical
Product description/Product definition properties:
ARGUS V60 sensor barriers are particularly compact and
Name Value Unit
strikingly elegant. Despite a housing depth of only 240 mm, the
Lock height 1200 mm
Argus V60 isa full-performance sensor barrier ideal for use
where space is limited. The reader units can be installed the Lock length 240 mm
same way as other versions of the Argus product range. Passage width 650 mm
Total width 1161 mm
The Argus sensor barriers are available in four versions; the
Power supply 300 VA
Argus 40 with a length of 1.200 mm, Argus 60 at 1.600 mm,
Argus 80 at 1.660 mm and the new Argus V60, particularly Performance data of the product with respect to its
compact at only 240 mm, for use in areas with constrained characteristics in accordance with the relevant technical
space requirements. provision which can be applied are mentioned above.
For the use and application of the product the respective Base materials/Ancillary materials
national provisions at the place of use apply. For ARGUS V60 The major material composition including the packaging of the
the standards which can be applied are the following: ARGUS V60 is listed below:
• Machinery Directive 2006/42/EC Name Value Unit
• 2014/30/EU Electromagnetic Compatibility Directive Aluminium 49 %
• 2011/65/EU ROHS2 Directive
Glass 29 %
• ISO 12100:2011-03 Safety of machinery
Paper 8 %
• EN 16005: 2013-01 and Amendment
Stainless steel 4 %
2015-10 Power operated pedestrian doorsets
• ISO 13849- 1:2016-06 Safety of machinery Steel 4 %
• ISO 13849- 2:2013-02 Safety of machinery Plastic 3 %
• EN 60335-2-103: 2016-05 Household and similar Zinc 2 %
electrical appliances
Electronics 1 %
• EN 61000-3-2:2015-03 Electromagnetic compatibility
(EMC) The product contains partial articles which contain substances
• EN 61000-6-2: 2005 and Amendment:2011 listed in the Candidate List of REACH Regulation
Electromagnetic Compatibility (EMC) 1907/2006/EC (date: 17.01.2023) exceeding 0.1 percentage by
• EN 61000-6-3:2007 and A1:2011 Electromagnetic mass: yes
Compatibility (EMC) • Lead (Pb): 7439-921 -1 (CAS-No.) is included in some
The CE-marking takes into account the proof of conformity with of the alloys used. The concentration of lead in each
the respective harmonized standards based on the legal individual alloy does not exceed 4 % (by mass).
provisions above. The Candidate List can be found on the /ECHA/ website
address: https://echa.europa.eu/de/home.
Application
For reliabable security, ideal for use where space is limited like: Reference service life
• Offices The reference service life of the ARGUS V60 amounts to 15
• Business rooms years and depends on the application and frequency of use.
• Company sites Regular maintenance is advised to ensure the life expectancy
• Entrances of 15 years. For repairs or renewals, suitable spare part are
• Educational centres available. The ARGUS V60 is tested andf certified to EN 16005,
meaning they are designed to withstand a minimum of 500.000
Technical Data cycles .
LCA: Calculation rules
The product stage includes:
Declared Unit — A1, raw material extraction, processing and mechanical
treatments, processing of secondary material input (e.g.
The declared unit is 1 piece of product: ARGUS V60 recycling processes),
Name Value Unit — A2, transport to the manufacturer,
— A3, manufacturing and assembly including provision of all
Declared unit 1 pce.
materials, products and energy, as well as waste processing up
Mass on declared product 272.77 kg
to the end-of waste state.
Construction stage - Modules A4-A5
System boundary
The construction process stage includes:
Type of EPD: cradle to gate with options, modules C1–C4, and — A4, transport to the building site;
module D (A1–A3 + C + D and additional modules: A4 + A5 + — A5, installation into the building; including provision of all
B6) materials, products and energy, as well as waste processing up
to the end-of-waste state or disposal of final residues during the
Production - Module A1-A3 construction process stage.
2 Environmental Product Declaration - dormakaba - ARGUS V60
— D, recycling potentials, expressed as net impacts and
Use stage - Module B6 benefits.
The use stage related to the operation of the building includes:
— B6, operational energy use The potential use of electricity Geographic Representativeness
from the grid is declared in module B6. Land or region, in which the declared product system is
manufactured, used or handled at the end of the product´s
End-of-life stage– Modules C1-C4 and D lifespan: Global
The end-of-life stage includes:
— C1, de-construction, demolition:
Comparability
— C2, transport to waste processing;
Basically, a comparison or an evaluation of EPD data is only
— C3, waste processing for reuse, recovery and/or recycling;
possible if all the data sets to be compared were created
— C4, disposal; including provision and all transport, provision
according to EN 15804 and the building context, respectively
of all materials, products and related energy and water use.
the product-specific characteristics of performance, are taken
into account. Background database: GaBi ts , SP40.
Module D (Benefits and loads beyond the system boundary)
includes:
LCA: Scenarios and additional technical information
Name Value Unit
Characteristic product properties of biogenic carbon
Days per year in use 365 days
On mode per day 1,1 hours
Information on describing the biogenic Carbon Content at
Idle mode per day 22,9 hours
factury gate
On mode power 31 W
Name Value Unit
Idle mode power 17 W
Biogenic carbon content in product 1.69 kg C
Electricity consumption per 1 year 154,54 kWh
Additional technical information for the declared modules. End of life (C1-C4)
Transport to the building site (A4) C1: The product dismantling from the building is done manually
without environmental burden.
Name Value Unit
Name Value Unit
Litres of fuel (per 1 kg) 0.00276l/100km
Collected separately waste type 256 kg
Transport distance via medium truck 100 km
Recycling 164 kg
Capacity utilisation (including empty runs) via
medium truck 55 % Energy recovery 4.46 kg
Landfilling 87.5 kg
The product is transported via truck. The main distribution
Transport to waste management 50 km
region is Europe. Transport distance is declared for a distance
of 100 km by truck in order to allow scaling to a specific point of The product is disassembled in a recycling process.
installation. Material recycling is then assumed for the metals, electronic
and electromechanics. The plastic components are assumed to
be incinerated with energy recovery. Minor proportions of
Installation into the building (A5) residues arising from the recycling process are landfilled.
Region for the End of Life is: Europe.
Name Value Unit
Waste packaging (paper and plastic) 16,9 kg
Reuse, recovery and/or recycling potentials (D), relevant
scenario information
Reference service life Name Value Unit
Name Value Unit Recycling 100 %
Life Span according to the manufacturer 15 a
The collection rate is 100%.
Operational energy use (B6)
3 Environmental Product Declaration - dormakaba - ARGUS V60
LCA: Results
DESCRIPTION OF THE SYSTEM BOUNDARY (X = INCLUDED IN LCA; MND = MODULE OR INDICATOR NOT DECLARED; MNR
= MODULE NOT RELEVANT)
Benefits and
Construction loads beyond
Product stage Use stage End of life stage
process stage the system
boundaries
la ire ta m w a Ry lp p u s tro p s n a rT g n iru tc a fu n a M e h t m o rf tro p s n a rTe tis e h t o t e ta g y lb m e s s A e s U e c n a n e tn ia M ria p e R tn e m e c a lp e R tn e m h s ib ru fe R y g re n e la n o ita re p Oe s u re ta w la n o ita re p Oe s u n o itc u rts n o c -e Dn o itilo m e d tro p s n a rT g n is s e c o rp e ts a W la s o p s iD -e s u e R-y re v o c e R-g n ilc y c e Rla itn e to p
A1 A2 A3 A4 A5 B1 B2 B3 B4 B5 B6 B7 C1 C2 C3 C4 D
X X X X X MND MND MNR MNR MNR X MND X X X X X
RESULTS OF THE LCA - ENVIRONMENTAL IMPACT according to EN 15804+A2: 1 piece ARGUS V60
Parameter Unit A1-A3 A4 A5 B6 C1 C2 C3 C4 D
GWP-total kg CO 2 eq 6.17E+02 2.39E+00 2.72E+01 9.38E+02 0 1.13E+00 1.97E+01 1.34E+00 -2.53E+02
GWP-fossil kg CO 2 eq 6.45E+02 2.28E+00 7.87E+00 9.33E+02 0 1.08E+00 1.15E+01 1.33E+00 -2.52E+02
GWP-biogenic kg CO 2 eq -2.85E+01 1.05E-01 1.94E+01 3.11E+00 0 5E-02 8.25E+00 5E-03 -3.59E-01
GWP-luluc kg CO 2 eq 5.28E-01 5.43E-05 7.43E-04 1.35E+00 0 2.56E-05 7.21E-04 4E-03 -1.5E-01
ODP kg CFC11 eq 1.34E-08 2.41E-16 7.3E-15 2.05E-11 0 1.14E-16 6.74E-15 4.92E-15 -1.34E-09
AP mol H+ eq 3.74E+00 2E-03 7E-03 2.06E+00 0 1E-03 3E-03 1E-02 -1.02E+00
EP-freshwater kg P eq 1.39E-03 4.88E-07 1.29E-06 2E-03 0 2.3E-07 1.06E-06 2.28E-06 -2E-04
EP-marine kg N eq 6.4E-01 7.26E-04 2E-03 4.58E-01 0 3.43E-04 8.45E-04 2E-03 -1.39E-01
EP-terrestrial mol N eq 7.04E+00 8E-03 3.1E-02 4.81E+00 0 4E-03 1.5E-02 2.7E-02 -1.5E+00
kg NMVOC
POCP 1.72E+00 2E-03 6E-03 1.25E+00 0 9.69E-04 2E-03 7E-03 -4.37E-01
eq
ADPE kg Sb eq 7.41E-02 6.84E-08 1.08E-07 2.7E-04 0 3.23E-08 9.46E-08 1.19E-07 -1.2E-02
ADPF MJ 8.49E+03 3.23E+01 9.68E+00 1.64E+04 0 1.53E+01 7.05E+00 1.74E+01 -3.52E+03
m3 world eq
WDP 1.17E+02 4E-03 3.22E+00 2.03E+02 0 2E-03 2.02E+00 1.39E-01 -3.45E+01
deprived
GWP = Global warming potential; ODP = Depletion potential of the stratospheric ozone layer; AP = Acidification potential of land and water; EP =
Eutrophication potential; POCP = Formation potential of tropospheric ozone photochemical oxidants; ADPE = Abiotic depletion potential for non-fossil
resources; ADPF = Abiotic depletion potential for fossil resources; WDP = Water (user) deprivation potential)
RESULTS OF THE LCA - INDICATORS TO DESCRIBE RESOURCE USE according to EN 15804+A2: 1 piece ARGUS V60
Parameter Unit A1-A3 A4 A5 B6 C1 C2 C3 C4 D
PERE MJ 2.72E+03 1.02E-01 1.7E+02 7.27E+03 0 4.8E-02 5.69E+01 2.28E+00 -1.37E+03
PERM MJ 2.23E+02 0 -1.68E+02 0 0 0 -5.52E+01 0 0
PERT MJ 2.94E+03 1.02E-01 2.03E+00 7.27E+03 0 4.8E-02 1.7E+00 2.28E+00 -1.37E+03
PENRE MJ 8.2E+03 3.24E+01 1.34E+02 1.64E+04 0 1.53E+01 1.79E+02 1.74E+01 -3.52E+03
PENRM MJ 2.97E+02 0 -1.25E+02 0 0 0 -1.72E+02 0 0
PENRT MJ 8.49E+03 3.24E+01 9.69E+00 1.64E+04 0 1.53E+01 7.05E+00 1.74E+01 -3.52E+03
SM kg 1.2E+02 0 0 0 0 0 0 0 0
RSF MJ 0 0 0 0 0 0 0 0 0
NRSF MJ 0 0 0 0 0 0 0 0 0
FW m3 5.89E+00 1.83E-04 7.6E-02 8.41E+00 0 8.63E-05 4.8E-02 4E-03 -2.99E+00
PERE = Use of renewable primary energy excluding renewable primary energy resources used as raw materials; PERM = Use of renewable primary
energy resources used as raw materials; PERT = Total use of renewable primary energy resources; PENRE = Use of non-renewable primary energy
excluding non-renewable primary energy resources used as raw materials; PENRM = Use of non-renewable primary energy resources used as raw
materials; PENRT = Total use of non-renewable primary energy resources; SM = Use of secondary material; RSF = Use of renewable secondary fuels;
NRSF = Use of non-renewable secondary fuels; FW = Use of net fresh water
RESULTS OF THE LCA – WASTE CATEGORIES AND OUTPUT FLOWS according to EN 15804+A2:
1 piece ARGUS V60
Parameter Unit A1-A3 A4 A5 B6 C1 C2 C3 C4 D
HWD kg 1.15E-04 3.14E-09 2.23E-08 6.79E-06 0 1.48E-09 2.13E-08 2.66E-07 -1.32E-05
NHWD kg 9.04E+01 3E-03 1.39E+00 1.16E+01 0 2E-03 1.24E+00 8.76E+01 -4.92E+01
RWD kg 3.22E-01 3.47E-05 4.56E-04 2.49E+00 0 1.64E-05 2.98E-04 1.98E-04 -3.04E-01
CRU kg 0 0 0 0 0 0 0 0 0
MFR kg 0 0 0 0 0 0 5.25E+01 0 0
MER kg 0 0 0 0 0 0 0 0 0
EEE MJ 0 0 4.37E+01 0 0 0 3.53E+01 0 0
EET MJ 0 0 8.58E+01 0 0 0 7.52E+01 0 0
4 Environmental Product Declaration - dormakaba - ARGUS V60
HWD = Hazardous waste disposed; NHWD = Non-hazardous waste disposed; RWD = Radioactive waste disposed; CRU = Components for re-use;
MFR = Materials for recycling; MER = Materials for energy recovery; EEE = Exported electrical energy; EET = Exported thermal energy
RESULTS OF THE LCA – additional impact categories according to EN 15804+A2-optional:
1 piece ARGUS V60
Parameter Unit A1-A3 A4 A5 B6 C1 C2 C3 C4 D
Disease
PM 3.59E-05 1.2E-08 4.75E-08 1.73E-05 0 5.66E-09 3.18E-08 1.18E-07 -1.65E-05
incidence
IR kBq U235 eq 5.43E+01 5E-03 6.2E-02 4.08E+02 0 2E-03 3.4E-02 2E-02 -5.94E+01
ETP-fw CTUe 5.17E+03 2.29E+01 4.26E+00 7.02E+03 0 1.08E+01 2.76E+00 9.95E+00 -1.4E+03
HTP-c CTUh 1.62E-05 4.31E-10 2.68E-10 1.94E-07 0 2.04E-10 2.23E-10 1.47E-09 -7.98E-08
HTP-nc CTUh 1.13E-05 1.84E-08 1.81E-08 7.14E-06 0 8.7E-09 1.91E-08 1.63E-07 6.57E-06
SQP SQP 4.37E+03 8.3E-02 2.69E+00 5.22E+03 0 3.9E-02 2.07E+00 3.63E+00 -2.32E+02
PM = Potential incidence of disease due to PM emissions; IR = Potential Human exposure efficiency relative to U235; ETP-fw = Potential comparative
Toxic Unit for ecosystems; HTP-c = Potential comparative Toxic Unit for humans (cancerogenic); HTP-nc = Potential comparative Toxic Unit for humans
(not cancerogenic); SQP = Potential soil quality index
Disclaimer 1 – for the indicator “Potential Human exposure efficiency relative to U235”. This impact category deals mainly with the
eventual impact of low-dose ionizing radiation on human health of the nuclear fuel cycle. It does not consider effects due to possible
nuclear accidents, occupational exposure or radioactive waste disposal in underground facilities. Potential ionizing radiation from the
soil, radon and from some construction materials is also not measured by this indicator.
Disclaimer 2 – for the indicators “abiotic depletion potential for non-fossil resources”, “abiotic depletion potential for fossil resources”,
“water (user) deprivation potential, deprivation-weighted water consumption”, “potential comparative toxic unit for ecosystems”,
“potential comparative toxic unit for humans – cancerogenic”, “Potential comparative toxic unit for humans - not cancerogenic”,
“potential soil quality index”. The results of this environmental impact indicator shall be used with care as the uncertainties on these
results are high as there is limited experience with the indicator.
This EPD was created using a software tool.
References
ISO 14025 ISO 9001:201509 Quality management systems Requirements
ISO 14025:2011-10, Environmental labels and declarations —
Type III environmental declarations — Principles and Machinery Directive
procedures DIRECTIVE 2006/42/EC OF THE EUROPEAN PARLIAMENT
AND OF THE COUNCILof 17 May 2006on machinery, and
EN 15804 amending Directive 95/16/EC
EN 15804:2019+AC:2021, Sustainability of construction works
— Environmental Product Declarations — Core rules for the REACH
product category of construction products Regulation (EC) No 1907/2006 of the European Parliament and
of the Council on the Registration, Evaluation, Authorisation
EN 16005 and Restriction of Chemicals (REACH)
EN 16005: 201301 and Amendment 2015-10 Power operated
pedestrian doorsets 2011/65/EU ROHS3 Directive
Directive 2011/65/EU of the European Parliament and of the
EN 60335-2 Council of 8 June 2011 on the restriction of the use of certain
EN 603352103: 201605 Household and similar electrical hazardous substances in electrical and electronic equipment
appliances
Further References
EN 61000-3-2
EN 6100032: 201503 Electromagnetic compatibility (EMC) IBU 2021
General Instructions for the EPD programme of Institut Bauen
EN 61000-6-2 und Umwelt e.V. Version 2.0, Berlin: Institut Bauen und Umwelt
EN 6100062: 2005 and Amendment:2011 Electromagnetic e.V., 2021. www.ibu-epd.com
Compatibility (EMC)
GaBi
EN 61000-6-3 Sphera Solutions GmbH Gabi Software System and Database
EN 6100063: 2007 and A1:2011 Electromagnetic Compatibility for Life Cycle Engineering 19922020 Version 10.0.0.71
(EMC) University of Stuttgart Leinfelden-Echterdingen
ISO 12100 GaBi ts documentation
ISO 12100:201103 Safety of machinery GaBi life cycle inventory data documentation
(https://www.gabisoftware.
ISO 13849- 1 com/support/gabi/gabidatabase[1]2020lcidocumentation/).
ISO 138491: 201606 Safety of machinery
LCA-tool dormakaba
ISO 13849- 2 LCA tool, ESC (Entrance System Control) Tool No.: IBU-DOR-
ISO 138492: 201302 Safety of machinery 202109-LT1-EN Developed by Sphera Solutions GmbH.
ISO 9001 PCR Part A
5 Environmental Product Declaration - dormakaba - ARGUS V60
PCR – Part A: Calculation Rules for the Life Cycle Assessment PCR Part B
and Requirements on the Project Report according to EN PCR – Part B: Requirements on the EPD for electronic and
15804+A2:2019, Version 1.0, Institut Bauen und Umwelt e.V., physical Access Control Systems, version 08/21, Institut Bauen
www.ibu-epd.com. und Umwelt e.V., www.ibu-epd.com.
6 Environmental Product Declaration - dormakaba - ARGUS V60
Publisher
Institut Bauen und Umwelt e.V. +49 (0)30 3087748- 0
Hegelplatz 1 info@ibu-epd.com
10117 Berlin www.ibu-epd.com
Germany
Programme holder
Institut Bauen und Umwelt e.V. +49 (0)30 3087748- 0
Hegelplatz 1 info@ibu-epd.com
10117 Berlin www.ibu-epd.com
Germany
Author of the Life Cycle Assessment
dormakaba International Holding GmbH +49 2333 793-0
DORMA Platz 1 info.de@dormakaba.com
58256 Ennepetal www.dormakaba.com
Germany
Owner of the Declaration
dormakaba International Holding GmbH +49 2333 793-0
DORMA Platz 1 info.de@dormakaba.com
58256 Ennepetal www.dormakaba.com
Germany
7 Environmental Product Declaration - dormakaba - ARGUS V60
