ENVIRONMENTAL PRODUCT DECLARATION
as per ISO 14025 and EN 15804+A2
Owner of the Declaration VIR – Valvoindustria Ing. Rizzio S.p.A.
Publisher Institut Bauen und Umwelt e.V. (IBU)
Programme holder Institut Bauen und Umwelt e.V. (IBU)
Declaration number EPD-VIR-20230494-IBC1-EN
Issue date 11/01/2024
Valid to 10/01/2029
Different brass valves family constituted by full bore ball valves,
gate valves and fixed-orifice balancing valves
Vir Valvoindustria Ing. Rizzio Spa
www.ibu-epd.com | https://epd-online.com
1. General Information
Vir Valvoindustria Ing. Rizzio Spa Different brass valves family constituted by full
bore ball valves, gate valves and fixed-orifice
balancing valves
Programme holder Owner of the declaration
IBU – Institut Bauen und Umwelt e.V. VIR – Valvoindustria Ing. Rizzio S.p.A.
Hegelplatz 1 Via circonvallazione 10
10117 Berlin 13018 Valduggia (VC)
Germany Italy
Declaration number Declared product / declared unit
EPD-VIR-20230494-IBC1-EN The declared unit is 1 kg of the average valve of the family
This declaration is based on the product category rules: Scope:
Fittings and connections for water supply, 01/08/2021 This Environmental Product Declaration refers to a declared unit of 1 kg of
(PCR checked and approved by the SVR) the average valve of the brass family - type '340' '56' and 'Serie 9510' -
produced at the production site of VIR - Valvoindustria Ing. Rizzio S.p.A. in
Via circonvallazione 10, 13018 Valduggia (VC), Italy.
Issue date The owner of the declaration shall be liable for the underlying information
and evidence; the IBU shall not be liable with respect to manufacturer
11/01/2024
information, life cycle assessment data and evidences.
The EPD was created according to the specifications of EN 15804+A2. In
Valid to
the following, the standard will be simplified as EN 15804.
10/01/2029
Verification
The standard EN 15804 serves as the core PCR
Independent verification of the declaration and data according to ISO
14025:2011
internally X externally
Dipl.-Ing. Hans Peters
(Chairman of Institut Bauen und Umwelt e.V.)
Florian Pronold Vito D'Incognito,
(Managing Director Institut Bauen und Umwelt e.V.) (Independent verifier)
Environmental Product Declaration - Vir Valvoindustria Ing. Rizzio Spa - Different brass valves family constituted by full bore ball valves, gate valves and fixed-orifice
1 balancing valves
2. Product
This product contains substances listed in the candidate list
2.1 Product description/Product definition (date: 14.06.2023) exceeding 0.1 percentage by mass:
The process starts with the manufacturing of raw brass pieces
• Lead (CAS 7439-92-1) - concentration range: 1.6% -
for valves obtained from casting and hot-moulding then the
2.8%.
pieces are mechanically worked and assembled with valves
components (e.g. handles, gaskets, balls, fittings, etc.). 2.6 Manufacture
Declared units refer to three different types of valves - 340, 56
and Serie 9510. Every valve typology contains valves with
different dimensions and weights. However, the same
manufacturing process and the similarities of valves allow a
declared unit based on a mass unit of products.
For the use and application of the product, the respective
national provisions at the place of use apply, in Germany for
example the building codes of the federal states and the
corresponding national specifications.
2.2 Application
Model 340: Water from 0°C to 150°C and air from -10°C to
150°C
Model 56: Water from 0°C to 150°C
Model 9510: Water from -10°C to 130°C
2.3 Technical Data
The valves are tested according to EN 12266-1 standard.
Technical data
Name Value Unit
medium Water, air
Nominal diameter (DN) 10 - 100
Weight 0.00009 - 0.0086 t
Housing material Brass
spindle material Brass
2.7 Environment and health during manufacturing
Performance data of the product with respect to its
The manufacturing stage is made in accordance with the Italian
characteristics are in accordance with the relevant technical
regulation.
provision.
2.8 Product processing/Installation
2.4 Delivery status
The valves are delivered fully assembled, tested, and packaged 1. BLASTING: the brass pieces are subjected to a surface
with a plastic envelope and a carton box, to Italy and to the rest treatment by a sandblasting machine and steel grit;
of the World (mainly where manufacturer's branches are 2. TURNING: the valves are machined by transfer
located). For land transport the products are delivered by machines or numerical control machining centres (CNC)
trucks, while for sea routes they are transported by cargo ships. cooled by cooling oil. The brass turning is dried by
centrifuge and conveyed to a silo for sale as a
2.5 Base materials/Ancillary materials
secondary raw material;
Name Value Unit 3. ASSEMBLY: the valves are assembled by automatic
Brass 0.8373 kg machines by performing 100% air test and fixing the
components with adhesives;
Steel 0.0992 kg
4. PACKAGING AND STORAGE: following the quality
Aluminium 0.0162 kg
check, the valves are packaged ensuring adequate
ABS 0.0284 kg protection and stored for shipment.
PTFE 0.0094 kg
2.9 Packaging
Polypropylene 0.0031 kg
The packaging materials are the following:
Polyoxymethylene 0.0024 kg
EPDM rubber 0.0024 kg • Wood (7.3 %);
• Paper and cardboard (78.8 %);
NBR rubber 0.0008 kg
• Polyethylene (0.8 %);
Synthetic rubber 0.0008 kg
• Plastic film (13.1 %).
Environmental Product Declaration - Vir Valvoindustria Ing. Rizzio Spa - Different brass valves family constituted by full bore ball valves, gate valves and fixed-orifice
2 balancing valves
The disposal of the packaging is consistent with the regulation No impacts on the environment are expected in the case of an
of the countries of sale. unforeseeable mechanical destruction.
2.10 Condition of use 2.14 Re-use phase
No auxiliaries or consumables are incurred during With reference to the material composition of the product
maintenance, and use of the Valves. Regular maintenance is system in accordance with section 2.5, the metallurgical
advised to ensure a service life of at least 10 years. materials contained in the product are suitable for material
recycling.
2.11 Environment and health during use
There are no known impact relations between product, 2.15 Disposal
environment and health during use. If there is no specific regulation for the valve disposal, VIR
reccommends to:
2.12 Reference service life - Recycle the metal parts to reuse it as raw material;
Regular maintenance is advised to ensure a service life which - Send to specifical end-of-life guarantees and others PTFE
is minimum 10 years. (Polytetrafluoroethylene), NBR (Nitril-Butadiene-rubber) and
EPDM (ethylene propylene diene monomer rubber) elements,
2.13 Extraordinary effects
since they could be contaminated by the liquids flowing in the
Fire valve;
Due to the predominant use of brass and steel which are - Collect all the packaging to the local waste sorting system.
considered nonflammable or flame retardant, no additional
influence on the environment in case of fire is to be expected.
Water 2.16 Further information
Two water contaminants can be found into the valve: lead and Contact data for more detailed information: Please refer to the
nickel. last page of this Declaration
Mechanical destruction
3. LCA: Calculation rules
of the raw material.
3.1 Declared Unit
The functional unit is constituted as the weighted average 3.3 Estimates and assumptions
between the three type of valves. The mass of assembled The Brass used in the valves production was modelled
products corresponding to each family has been used as the assuming that it comes only from new material. In C2, the
weight of the average. distance between the use site and the disposal site is assumed
to be 50 km.
Deklarierte Einheit
Name Value Unit 3.4 Cut-off criteria
Declared unit 1 kg The effect associated with the neglected mass shares is less
Gross density 8460 kg/m3 than 5 % of the effect categories per module.
The use of an average EPD seems to be consistent due to the 3.5 Background data
low variability of the three type of valves. All the valves included The LCA software Simapro 9.5.0.1 was used to model the life
in the average are manufactured by the same producer, in the cycle. The entire manufacturing process, as well as energy
same plant, with the same manufacturing proccesses. Since consumption, were modelled on the basis of manufacturer
there is only one production site the modellization is highly specific data. However, generic background datasets were
geographically representative and background data have the used for the upstream and downstream processes. The
same inluence on all the considered type of valves. background datasets used were taken from the current version
of the Ecoinvent 3.9.1 database.
3.2 System boundary
Where possible, Italian datasets were used for modules A1-A3,
Type of the EPD: cradle to gate with options
A5, C1, C3, C4 and D; the corresponding European datasets
for distribution transports (A4, C2).
Modules A1-A3, A4 and A5
Here there is the production of the necessary raw materials and 3.6 Data quality
energies, including all corresponding upstream chains and the The background datasets used for accounting purposes mainly
actual procurement transports. Furthermore, the entire originate from the respective updated Ecoinvent 3.9.1
manufacturing phase was mapped, including the treatment of databases, through the software Simapro 9.5.0.1, at the time of
production waste until the endofwaste status (EoW) was calculation. The data for the examined products was captured
reached. In addition the distribution transports (A4) and the on the basis of evaluations of internal production and
installation (with also packaging waste generated during environmental data, the collection of LCA relevant data within
installation) was taken into account. the supply chain, as well as the evaluation of relevant data for
the energy supply. The collected data were checked for
Modules C1-C4 plausibility and consistency. Good representativity can be
The modules include the environmental impacts for dismantling assumed.
of the valve and the treatment of the waste categories until end-
of-waste status (EoW) is reached, including the associated 3.7 Period under review
transports at the end of the product life cycle. Life cycle assessment data refer to 2021.
Module D 3.8 Geographic Representativeness
Identification of the benefits and impacts of the product outside Land or region, in which the declared product system is
the system boundary. Recycling of metal scrap results in credits manufactured, used or handled at the end of the product´s
Environmental Product Declaration - Vir Valvoindustria Ing. Rizzio Spa - Different brass valves family constituted by full bore ball valves, gate valves and fixed-orifice
3 balancing valves
lifespan: Global
3.10 Comparability
Basically, a comparison or an evaluation of EPD data is only
3.9 Allocation possible if all the data sets to be compared were created
All raw materials, and supplies could be (clearly) assigned to according to EN 15804 and the building context, respectively
the declared product. All required energies, waste produced in the product-specific characteristics of performance, are taken
the manufacturing processes and production emissions are into account. The background database used is Ecoinvent
allocated to each family on the basis of the total mass of valves 3.9.1, through the software Simapro 9.5.0.1.
produced. No byproducts are produced or any other allocation
is needed.
4. LCA: Scenarios and additional technical information
Characteristic product properties of biogenic carbon The A1, A2, A3, C1, C2, C3, C4 and D stage have been
There is no biogenic carbon content in the product, while considered separately. The optional A4 and A5 stage have also
differently, the packaging has a non-zero amount. been considered.
Transport from the gate to the site (A4)
Note: 1 kg of biogenic carbon is equivalent to 44/12 kg of CO2.
Name Value Unit
Information on describing the biogenic carbon content at
Land transport distance 185.59 km
factory gate
Sea transport distance 1594.24 km
Name Value Unit
kg Regular maintenance is advised to ensure a service life of at
Biogenic carbon content in product - C least 10 years.
Biogenic carbon content in accompanying kg
0.1331
packaging C
Environmental Product Declaration - Vir Valvoindustria Ing. Rizzio Spa - Different brass valves family constituted by full bore ball valves, gate valves and fixed-orifice
4 balancing valves
5. LCA: Results
The following table shows the results of the LCA for 1kg of Brass Valve of the VIR models: 340, 56 and Serie 9510.
DESCRIPTION OF THE SYSTEM BOUNDARY (X = INCLUDED IN LCA; MND = MODULE OR INDICATOR NOT DECLARED; MNR
= MODULE NOT RELEVANT)
Benefits and
Construction loads beyond
Product stage Use stage End of life stage
process stage the system
boundaries
la ire ta m w a Ry lp p u s tro p s n a rT g n iru tc a fu n a M e h t m o rf tro p s n a rTe tis e h t o t e ta g y lb m e s s A e s U e c n a n e tn ia M ria p e R tn e m e c a lp e R tn e m h s ib ru fe R y g re n e la n o ita re p Oe s u re ta w la n o ita re p Oe s u n o itc u rts n o c -e Dn o itilo m e d tro p s n a rT g n is s e c o rp e ts a W la s o p s iD -e s u e R-y re v o c e R-g n ilc y c e Rla itn e to p
A1 A2 A3 A4 A5 B1 B2 B3 B4 B5 B6 B7 C1 C2 C3 C4 D
X X X X X MND MND MNR MNR MNR MND MND X X X X X
RESULTS OF THE LCA - ENVIRONMENTAL IMPACT according to EN 15804+A2: 1 kg Average Brass Valve
Parameter Unit A1-A3 A4 A5 C1 C2 C3 C4 D
GWP-total kg CO 2 eq 9.65E+00 5.1E-02 3.18E-02 0 9.43E-03 9.85E-02 4.87E-03 -2.69E+00
GWP-fossil kg CO 2 eq 9.59E+00 5.09E-02 7.54E-03 0 9.42E-03 5.71E-02 4.87E-03 -2.66E+00
GWP-biogenic kg CO 2 eq 1.87E-01 1.14E-05 -7.69E-02 2.81E-05 2.43E-02 0 8.51E-06 4.13E-02
GWP-luluc kg CO 2 eq 2.29E-02 6.45E-06 1.12E-02 2.94E-05 3.14E-07 0 4.57E-06 1.43E-04
ODP kg CFC11 eq 3.34E-05 1E-09 1.78E-11 0 2.05E-10 7.51E-10 1.35E-11 -3.18E-08
AP mol H+ eq 3.8E-01 5.96E-04 5.72E-06 0 3.07E-05 3.92E-04 4.35E-06 -1.92E-01
EP-freshwater kg P eq 3.03E-02 2.97E-06 1.48E-07 0 6.59E-07 1.27E-05 8.55E-08 -1.52E-02
EP-marine kg N eq 2.27E-02 1.59E-04 1.49E-05 0 1.06E-05 1.55E-04 1.03E-04 -1.01E-02
EP-terrestrial mol N eq 2.91E-01 1.74E-03 2.54E-05 0 1.11E-04 1.37E-03 1.67E-05 -1.37E-01
kg NMVOC
POCP 8.5E-02 5.29E-04 8.45E-06 0 4.59E-05 4.38E-04 6.77E-06 -3.87E-02
eq
ADPE kg Sb eq 5.07E-03 1.27E-07 1.28E-09 0 3.02E-08 4.89E-07 1.3E-09 -2.64E-03
ADPF MJ 1.16E+02 6.91E-01 7.81E-03 0 1.33E-01 6.78E-01 1.26E-02 -3.37E+01
m3 world eq
WDP 6.63E+00 2.45E-03 4.57E-04 0 5.44E-04 5.46E-03 5.21E-04 -3.05E+00
deprived
GWP = Global warming potential; ODP = Depletion potential of the stratospheric ozone layer; AP = Acidification potential of land and water; EP =
Eutrophication potential; POCP = Formation potential of tropospheric ozone photochemical oxidants; ADPE = Abiotic depletion potential for non-fossil
resources; ADPF = Abiotic depletion potential for fossil resources; WDP = Water (user) deprivation potential)
RESULTS OF THE LCA - INDICATORS TO DESCRIBE RESOURCE USE according to EN 15804+A2: 1 kg Average Brass Valve
Parameter Unit A1-A3 A4 A5 C1 C2 C3 C4 D
PERE MJ 1.48E+01 5.65E-03 1.32E-04 0 1.29E-03 1.3E-02 1.77E-04 -7.02E+00
PERM MJ 1.01E+01 3.42E-03 9.32E-05 0 7.85E-04 1.94E-02 8.51E-05 -1.8E+00
PERT MJ 2.48E+01 9.07E-03 2.25E-04 0 2.07E-03 3.24E-02 2.62E-04 -8.82E+00
PENRE MJ 1.15E+02 6.91E-01 0 0 0 -1.84E-03 0 1.73E-02
PENRM MJ 3.89E-02 0 0 0 0 1.84E-03 0 -1.73E-02
PENRT MJ 1.16E+02 6.91E-01 0 0 0 0 0 0
SM kg ND ND ND ND ND ND ND ND
RSF MJ ND ND ND ND ND ND ND ND
NRSF MJ ND ND ND ND ND ND ND ND
FW m3 6.77E+00 2.45E-03 4.54E-04 0 5.42E-04 5.47E-03 5.21E-04 -3.13E+00
PERE = Use of renewable primary energy excluding renewable primary energy resources used as raw materials; PERM = Use of renewable primary
energy resources used as raw materials; PERT = Total use of renewable primary energy resources; PENRE = Use of non-renewable primary energy
excluding non-renewable primary energy resources used as raw materials; PENRM = Use of non-renewable primary energy resources used as raw
materials; PENRT = Total use of non-renewable primary energy resources; SM = Use of secondary material; RSF = Use of renewable secondary fuels;
NRSF = Use of non-renewable secondary fuels; FW = Use of net fresh water
RESULTS OF THE LCA – WASTE CATEGORIES AND OUTPUT FLOWS according to EN 15804+A2:
1 kg Average Brass Valve
Parameter Unit A1-A3 A4 A5 C1 C2 C3 C4 D
HWD kg 2.9E-03 4.12E-06 3.93E-08 0 8.5E-07 3.9E-06 6.13E-08 -1.4E-03
NHWD kg 2.46E+00 2.46E-02 1.75E-02 0 6.52E-03 3.26E-02 4.81E-02 -1.06E+00
RWD kg 2.83E-04 1.82E-07 3.49E-09 0 4.34E-08 3.65E-07 4.79E-09 -8.75E-05
CRU kg 0 0 0 0 0 0 0 0
MFR kg 0 0 0 0 0 6.06E-01 0 0
MER kg 0 0 5.5E-03 0 0 0 0 0
EEE MJ 0 0 0 0 0 0 0 0
EET MJ 0 0 0 0 0 0 0 0
Environmental Product Declaration - Vir Valvoindustria Ing. Rizzio Spa - Different brass valves family constituted by full bore ball valves, gate valves and fixed-orifice
5 balancing valves
HWD = Hazardous waste disposed; NHWD = Non-hazardous waste disposed; RWD = Radioactive waste disposed; CRU = Components for re-use;
MFR = Materials for recycling; MER = Materials for energy recovery; EEE = Exported electrical energy; EET = Exported thermal energy
RESULTS OF THE LCA – additional impact categories according to EN 15804+A2-optional:
1 kg Average Brass Valve
Parameter Unit A1-A3 A4 A5 C1 C2 C3 C4 D
Disease
PM ND ND ND ND ND ND ND ND
incidence
IR kBq U235 eq ND ND ND ND ND ND ND ND
ETP-fw CTUe ND ND ND ND ND ND ND ND
HTP-c CTUh ND ND ND ND ND ND ND ND
HTP-nc CTUh ND ND ND ND ND ND ND ND
SQP SQP ND ND ND ND ND ND ND ND
PM = Potential incidence of disease due to PM emissions; IR = Potential Human exposure efficiency relative to U235; ETP-fw = Potential comparative
Toxic Unit for ecosystems; HTP-c = Potential comparative Toxic Unit for humans (cancerogenic); HTP-nc = Potential comparative Toxic Unit for humans
(not cancerogenic); SQP = Potential soil quality index
Disclaimer 1 – for the indicator “Potential Human exposure efficiency relative to U235”. This impact category deals mainly with the
eventual impact of low-dose ionizing radiation on human health of the nuclear fuel cycle. It does not consider effects due to possible
nuclear accidents, occupational exposure or radioactive waste disposal in underground facilities. Potential ionizing radiation from the
soil, radon and from some construction materials is also not measured by this indicator.
Disclaimer 2 – for the indicators “abiotic depletion potential for non-fossil resources”, “abiotic depletion potential for fossil resources”,
“water (user) deprivation potential, deprivation-weighted water consumption”, “potential comparative toxic unit for ecosystems”,
“potential comparative toxic unit for humans – cancerogenic”, “Potential comparative toxic unit for humans - not cancerogenic”,
“potential soil quality index”. The results of this environmental impact indicator shall be used with care as the uncertainties on these
results are high as there is limited experience with the indicator.
6. LCA: Interpretation
Specifically, the main impacts are in the A1 and A3 modules
The EN 15804 characterization factors were used for the and they are generated by the material production, while the
evaluation. The results of the EN 15804 categories refer to the transport related modules impacts are very low (A2 and A4).
potential environmental impacts over a period of 100 years. The negative value related to GWP - Biogenic refers to the
The main impacts clearly come from A1 - A3 stages while the presence of wood in the packaging.
end-of-life (C1-C4) stages results show to have low relevance.
7. Requisite evidence
Environmental Product Declaration - Vir Valvoindustria Ing. Rizzio Spa - Different brass valves family constituted by full bore ball valves, gate valves and fixed-orifice
6 balancing valves
8. References
Standards procedures.
EN 15804 Further References
EN 15804:2012+A1 2013, Sustainability of construction works
— Environmental Product Declarations — Core rules for the SimaPro
product category of construction products. SimaPro software and databases. Version 9.4.0.2, PRè
Sustainability B.V. https://simapro.com/, 2023.
EN 15804
EN 15804:2012+A2:2019+AC:2021, Sustainability of Ecoinvent Version 3.8
construction works — Environmental Product Declarations — Database for life cycle assessment (life cycle inventory data),
Core rules for the product category of construction products. Version 3.8, 2021.
EN 12266-1 Product Category Rules Part A
EN 12266-1:2012, Industrial valves - Testing of metallic valves - Calculation Rules for the Life Cycle Assessment and
Part 1: Pressure tests, test procedures and acceptance Requirements on the Project Report. Version 2.1 (17.11.2021).
criteria - Mandatory requirements.
Product Category Rules Part B
ISO 14025 Requirements on the EPD for Fittings and connections for
EN ISO 14025:2011, Environmental labels and declarations — water supply. Version 5 (31.05.2023).
Type III environmental declarations — Principles and
Environmental Product Declaration - Vir Valvoindustria Ing. Rizzio Spa - Different brass valves family constituted by full bore ball valves, gate valves and fixed-orifice
7 balancing valves
Publisher
Institut Bauen und Umwelt e.V. +49 (0)30 3087748- 0
Hegelplatz 1 info@ibu-epd.com
10117 Berlin www.ibu-epd.com
Germany
Programme holder
Institut Bauen und Umwelt e.V. +49 (0)30 3087748- 0
Hegelplatz 1 info@ibu-epd.com
10117 Berlin www.ibu-epd.com
Germany
Author of the Life Cycle Assessment
ICIM Consulting srl +39 02 72534800
Piazza Don Enrico Mapelli 75 info@icimconsulting.it
20099 Sesto San Giovanni www.icimconsulting.it
Italy
Owner of the Declaration
VIR – Valvoindustria Ing. Rizzio S.p.A. +39016347891
Via circonvallazione 10 info@vironline.com
13018 Valduggia (VC) www.vironline.com
Italy
Environmental Product Declaration - Vir Valvoindustria Ing. Rizzio Spa - Different brass valves family constituted by full bore ball valves, gate valves and fixed-orifice
8 balancing valves
