Environmental Product
Declaration
as per ISO 14025 and EN 15804
Owner of the declaration: Vaillant GmbH
Publisher: Kiwa-Ecobility Experts
Programme operator: Kiwa-Ecobility Experts
Registration number: EPD-Kiwa-EE-000271-EN
Issue date: 13.03.2024
Valid until: 13.03.2029
aroTHERM plus 5 kW & uniTOWER plus
The aroTHERM plus 5 kW is also known as “VWL 55/6 A 230V S2”, which is the outdoor unit of an
air-to-water heat pump with monobloc technology. The uniTOWER plus is also known as „VIH QW
190/6 E”, which is the indoor unit of an air-to-water heat pump with monobloc technology.
1. General information
Vaillant GmbH aroTHERM plus 5 kW & uniTOWER plus
Programme operator: Owner of the declaration:
Kiwa-Ecobility Experts Vaillant GmbH
Kiwa GmbH, Ecobility Experts Berghauser Straße 40
Wattstraße 11-13 42859 Remscheid
13355 Berlin Germany
Germany
Registration number: Declared product / declared unit:
EPD-Kiwa-EE-000271-EN 1 piece of heat pump system
Product category rules: Scope:
PCR A: General Product Category Rules for This Environmental Product Declararion (EPD)
Construction Products from the EPD program is based on the life cycle assessment (LCA) of
of Kiwa-Ecobility Experts; Version 2.1 the aroTHERM plus 5 kW (VWL 55/6 A 230V
S2) and the uniTOWER plus (VIH QW 190/6 E)
PCR B: PCR Guidance-Texts for Building-Re- produced by Vaillant. The used geographical
lated Products and Services: From the range area is Europe.
of Environmental Product Declarations of In-
stitute Construction and Environment e.V. The owner of the declaration shall be liable
(IBU) – Part B: Requirements on the EPD for for the underlying information and evidence.
HVAC Appliances (18.08.2023) Kiwa-Ecobility Experts shall not be liable with
respect to manufacturer information, life cy-
Issue date: cle assessment data and evidences.
13.03.2024
Valid until:
13.03.2029
Verification:
The European standard EN 15804+A2:2019
serves as the core PCR.
Independent verification of the declaration
and data according to ISO 14025:20010.
☐internally ☒externally
Raoul Mancke
(Head of programme operations, Kiwa-Ecobility Ex-
perts)
Martin Koehrer Anne Kees Jeeninga
(Verification body, Kiwa-Ecobility Experts) (Third-party verifier)
Vaillant – aroTHERM plus 5 kW & uniTOWER plus | Page 2
2. Product
2.1 Product description
In Figure 1 the structure of a typical heat pump system with monobloc technology is shown.
Figure 1: Structure of a typical heat pump system with monobloc technology
It contains the following components:
(1) Outdoor unit
(2) eBUS line
(3) System controller
(4) Indoor unit controller
(5) Indoor unit with hot water tank
(6) Heating circuit
The aroTHERM plus 5 kW is also known as “VWL 55/6 A 230V S2”. The product is the outdoor unit of
an air-to-water heat pump with monobloc technology. The heat pump has a closed refrigerant circuit
in which a refrigerant circulates. Through cyclic evaporation, compression, condensation and expan-
sion, heat energy is absorbed from the environment and transferred to the building. In cooling mode,
heat energy is extracted from the building and released to the environment.
In Figure 2 the structure of the product aroTHERM plus 5 kW is shown.
Vaillant – aroTHERM plus 5 kW & uniTOWER plus | Page 3
Figure 2: Structure of the product aroTHERM plus 5 kW
It contains the following components:
(1) Air inlet grille
(2) Nameplate
(3) Air outlet grille
The uniTOWER plus is also known as „VIH QW 190/6 E”. This product is an indoor unit and system
controller should be used in combination with aroTHERM. In Figure 3 the structure of the product
uniTOWER plus is shown.
Vaillant – aroTHERM plus 5 kW & uniTOWER plus | Page 4
Figure 3: Structure of the product uniTOWER plus
It contains the following components:
(1) Front cover
(2) Recessed handle
(3) Operating elements
(4) Label with serial number on the rear
2.2 Raw materials
The raw materials for aroTHERM plus 5 kW are shown in Table 1.
Table 1: Mass percentages of the raw materials for aroTHERM plus 5 kW
Raw material Value Unit
Steel 61 m%
Copper 12 m%
Aluminium 7 m%
Vermiculite 4 m%
PET 4 m%
ABS 3 m%
Bitumen 2 m%
Others 7 m%
Vaillant – aroTHERM plus 5 kW & uniTOWER plus | Page 5
The raw materials for uniTOWER plus are shown in Table 2.
Table 2: Mass percentages of the raw materials for uniTOWER plus
Raw material Value Unit
Steel 86% m%
Copper 4% m%
PU 3% m%
Brass 2% m%
Others 6% m%
2.3 Technical data
The technical data for aroTHERM plus 5 kW (VWL 75/5 6 A 230V S2) are listed in Table 3.
Table 3: Technical data of aroTHERM plus 5 kW
Description Value Unit
Width 1100 mm
Height 765 mm
Depth 450 mm
Weight with packaging 146,4 kg
Weight without packaging 124,9 kg
Voltage 230 V
Frequency 50 Hz
Flow max 2300 m3/h
Head max 20 m
Nominal capacity 3,4 kW
Pumped liquid R290 -
The technical data for uniTOWER plus (VIH QW 190/6 E) are listed in Table 4.
Vaillant – aroTHERM plus 5 kW & uniTOWER plus | Page 6
Table 4: Technical data of uniTOWER plus
Description Value Unit
Width 595 mm
Height 1880 mm
Depth 693 mm
Weight with packaging 167,1 kg
Weight without packaging 147,4 kg
Voltage 230/400 V
Frequency 50 Hz
Rated power 8,6 kW
Rated current 23,5/13,6 A
2.4 Manufacturing
The assembly, manufacturing and functional test of aroTHERM plus 5 kW & uniTOWER plus takes place
at the production and development sites in Remscheid (Germany), Nantes (France) and Belper (United
Kingdom). In Figure 4 the process flow chart for aroTHERM plus 5 kW & uniTOWER plus is shown.
Figure 4: Process flow chart for aroTHERM plus 5 kW & uniTOWER plus
Vaillant – aroTHERM plus 5 kW & uniTOWER plus | Page 7
According to Vaillant there are the following assembly process steps for aroTHERM plus 5 kW &
uniTOWER plus:
• Pre-assembly of dedicated pre-assembly groups
• Transfer of Pre-assemled Modules to Final Assembly
• Final Assembly I
• Testing (High pressure test/ Helium Leakage Test)
• Final Assembly II
• Filling of appliances with Refrigerant
• Final Assembly III
• Testing (End of Line Test)
• Final Assembly IV
• Packaging
• Transport central storage
• Distribution
2.5 Reference service life
According to the PCR B, the reference service life (RSL) shall be in accordance with ISO 15686 if ap-
plicable. Since the RSL of heat pumps is not defined in ISO 15686, a reference service life (RSL) of 15
years is assumed in this EPD, which is confirmed by Vaillant as a valid realistic RSL.
2.6 Packaging
For the packaging of aroTHERM plus 5 kW EPS, paper, PE foil, Polyamide foil and wood are considered.
For the packaging of uniTOWER plus EPS, paper, PE foil, steel and wood are considered.
2.7 Other information
Further information on the product can be found on the manufacturer's website
(www.vaillant.com).
Vaillant – aroTHERM plus 5 kW & uniTOWER plus | Page 8
3. LCA: Calculation rules
3.1 Declared unit
According to the “PCR Guidance-Texts for Building-Related Products and Services – From the range of
Environmental Product Declarations of Institute Construction and Environment e.V. (IBU) – Part B: Re-
quirements on the EPD for HVAC Appliances” the declared unit is 1 piece of heat pump system.
Table 5: Declared unit
Description Value Unit
Declared unit 1 piece
Mass reference 313,5 kg/piece
Conversion factor to 1 kg 0,003189793 -
SCOP 5,7 -
Air flow (max. nominal volume) 2300 m3/h
E ”heating” 1228,1 kWh/a
E ”cooling” 428,9 kWh/a
3.2 System boundary
This EPD was created in accordance with DIN EN 15804+A2. It monitors the production phase, con-
struction phase, the use phase and the end-of-life phase as well as the benefits and loads beyond the
system boundary. According to DIN EN 15804 this corresponds to the product phases A1-A5, B1-B7,
C1-C4 and D. Therefore, the type of the EPD is “cradle to grave”.
The modules include:
• A1: Extraction of the raw materials
• A2: Transport of the raw material to the production site by the suppliers
• A3: Auxiliary materials and energy for the different processing steps; Production waste; Pack-
aging materials
• A4: Transport from the manufacturing site to the customers
• A5: According to the guide by Vaillant only human labour is needed for the construction/in-
stallation process and thus nothing is considered; Packaging waste
• B1: Emissions due to refrigerant leakage
• B2: Refill of refrigerant
• B3: The module “repair” is not considered during the use phase
• B4: The module “replacement” is not considered during the use phase
• B5: The module “refurbishment” is not considered during the use phase
• B6: Operational energy use is considered
• B7: Operational waster use is not considered during the use phase
• C1: According to the guide by Vaillant only human labour is needed for the de-construc-
tion/demolition process and thus nothing is considered
• C2: Transport for waste treatments based on NMD waste scenarios
• C3: Waste processing based on NMD waste scenarios
Vaillant – aroTHERM plus 5 kW & uniTOWER plus | Page 9
• C4: Disposal based on NMD waste scenarios
• D: Loads due to landfill, incineration and recycling; Benefits due to incineration and recycling
For the declared life phases, all inputs (raw materials, intermediate products, energy and auxiliary ma-
terials) as well as the waste produced were considered.
3.3 Estimates and assumptions
As the products consist of so many different components, Vaillant preferred to use a conservative
approach for the transport of their suppliers (module A2). Therefore, a distance of 3500 km by truck is
considered for all components from Europe and 1000 km by truck as well as 19000 km by transoceanic
freight ship for all components from Asia.
The total operation time per year in heating mode t was assumed to be 1400 hours while the total
heating
operation time per year in cooling mode was assumed to be 350 hours, according to the default active
mode duration listed in PSR-0013.
For the end-of-life, waste scenarios from the Dutch Nationale Milieudatabase (NMD) waste scenarios
were used.
The further assumptions are only included in the background report for data protection reasons.
3.4 Cut-off criteria
For process modules A1 to A3, all process-specific data were collected. All flows could be assigned
potential environmental impacts through the Ecoinvent database 3.6. Production, supply, disposal,
maintenance and end-of-life treatment of capital goods are included. In the used Ecoinvent database
3.6 infrastructure and capital goods are included. All flows that contribute more than 1% of the total
mass, energy or environmental impact of the system have been included in the LCA. It can be assumed
that the neglected processes contributed less than 5% to the impact categories considered. It is as-
sumed that the contribution of capital goods to each individual environmental impact category of the
module (A1-A3) is less than 5%.
As this EPD is not a declaration at company level, but a declaration at product level, capital goods for
the production site are not taken into account, nor are packaging materials for the raw and auxiliary
materials.
3.5 Period under review
All process-specific data were collected for the operating year 2021.
3.6 Comparability
In principle, a comparison or assessment of the environmental impact of different products is only
possible if they have been produced in accordance with EN 15804. For the assessment of comparabil-
ity, the following aspects in particular must be taken into account: PCR used, functional or declared
unit, geographical reference, definition of the system boundary, declared modules, data selection (pri-
mary or secondary data, background database, data quality), scenarios used for the use and disposal
phases, and the life cycle inventory (data collection, calculation methods, allocations, validity period).
Vaillant – aroTHERM plus 5 kW & uniTOWER plus | Page 10
3.7 Background data
All the background data is taken from the Ecoinvent database version 3.6 (2019). The life cycle was
modelled with the help of the EPD & LCA tool R<THiNK. Almost all consistent datasets contained in the
Ecoinvent database version 3.6 (2019) are documented and can be viewed in the online documenta-
tion.
3.8 Data quality
Overall, the quality of the data can be considered as good. In the operating data survey, all relevant
process-specific data could be collected. The data were provided by the manufacturer Vaillant.
Secondary data were taken from the Ecoinvent database version 3.6 (2019). The database is regularly
checked and thus complies with the requirements of DIN EN ISO 14044 (background data not older
than 10 years). The background data meets the requirements of EN 15804. The quantities of raw ma-
terials, consumables and supplies used as well as the energy consumption have been recorded and
averaged over the entire year of operation.
The general rule has been complied that specific data from specific production processes or average
data derived from specific processes must be given priority when calculating an EPD or Life Cycle As-
sessment. Data for processes that the manufacturer cannot influence or choose, were backed up with
generic data.
The selection of the best fitting data sets is based on research and the help of experts. The transport
distances for the waste treatments as well as the used environmental profiles for loads and benefits
are based on the data from the NMD.
3.9 Allocation
Specific information about allocations within the background data is included in the documentation of
the Ecoinvent datasets.
3.10 Data collection
The data collection was performed according to ISO 14044:2006, section 4.3.2. According to the target
definition, all significant input and output flows that occur in connection with the products under con-
sideration were identified and quantified. The inputs and outputs were attributed to the process in
which they occur. For the process stages A1, A2 and A3, the input and output streams could be clearly
assigned.
The results of the operational data collection can be seen in the following tables. In addition to the
process-specific data, the tables also provide information on the respective background data used.
3.11 Calculation methods
For the life cycle assessment, the calculation methods described in the ISO 14044:2006, section 4.3.3
have been applied. The evaluation is based on the phases in the system boundaries and the processes
contained therein.
3.12 Electricity mix and CO certificates
2
The electricity mix was chosen according to the geographic reference space and time reference. As
only the conventional electricity mix is used, no further energy sources were considered. The power
Vaillant – aroTHERM plus 5 kW & uniTOWER plus | Page 11
mix composition is based on the Ecoinvent database version 3.6 (2019). No CO certificates were
2
counted.
4. LCA: Scenarios and additional technical information
The following scenarios are used in this EPD.
The EPD should be representative for Europe and thus Vaillant decided to consider their three main
countries of use in Europe. Therefore, Germany, Italy and the United Kingdom are considered for the
transport to the customers in module A4. Based on the percentages of the sales figures and the pro-
duction locations, a distance of 754 km was calculated. The details can be found in the background
report of this EPD.
Table 6: A4 – Transport from manufacturing sites to customers
Value and Unit
Lorry (Truck), unspecified (default) | market group for
Vehicle type used for transport
(GLO)
Fuel type and consumption of vehicle not available
Distance 754 km
Capacity utilisation (including empty
50 % (loaded up and return empty)
returns)
Bulk density of transported products inapplicable
Volume capacity utilisation factor 1
For input flows, there are no significant environment impacts as a result of materials or energy used in
the construction stage (A5).
The following output flows leaving the system at module A5 are assumed.
Table 7: A5 – Assembly
Description Value Unit
Output materials as result of loss during construction 3 %
Output materials as result of waste processing of materials used for kg
0,000
installation/assembly at the building site
Output materials as result of waste processing of used packaging 38,912 kg
During the use stage carbon dioxide emissions to the air due to the annual refrigerant leakage of 2%,
which is market compliant, is considered. For this the mass of the refrigerant R290 of 0,6 kg is multi-
plied by the leakage rate of 2% and the Global Warming Potential (GWP) value of 3 kg CO e/kg [Huber,
2
2022].
Vaillant – aroTHERM plus 5 kW & uniTOWER plus | Page 12
Table 8: B1 – Use
Description Cycle (yr) Number of cycles Amount per cycle Total Amount Unit
Refrigerant leakage 1 15 36000 540000 mg
Also, the annual refill of refrigerant is considered by multiplying the R290 mass of 0.6 kg with 2%.
Table 9: B2 – Maintenance
Description Service cycle (yr) Number of cycles (n) Amount per cycle Total Amount Unit
Refrigerant refill 1 14 0,012 0,168 kg
The total energy consumed by the heat pump to operate is calculated as the combination of energy
absorbed to exchange heat in heating and cooling mode along product RSL according to the PCR B. The
annual operation energy use is 1656,99 kWh and the total operation energy use along RSL is 24854,88
kWh.
Table 10: B6 – Operational energy use
Value Unit
P 5 kW
heat, design
SCOP 5,7 -
T 1400 hours/a
heating
E 1228,07 kWh/a
heating
P 5 kW
cool, design
SEER 4,08 -
T 350 hours/a
cooling
E 428,92 kWh/a
cooling
E 24854,88 kWh
use
As already described in section 3.3, the following waste scenarios are from the Dutch Nationale Mi-
lieudatabase (NMD).
Table 11: C2 - Transport End-of-Life
Waste treatment Transport profile Transport distance [km]
Landfill Lorry (Truck), unspecified (default) 100
Incineration Lorry (Truck), unspecified (default) 150
Recycling Lorry (Truck), unspecified (default) 50
Vaillant – aroTHERM plus 5 kW & uniTOWER plus | Page 13
Table 12: Percentages of the waste treatments for the waste scenarios
Landfill Incinera- Recy- Reuse
Waste scenario
[%] tion [%] cling [%] [%]
aluminium, cast alloy for buildings (i.a. profiles, 0
3 3 94
sheets, pipes) (NMD ID 4)
bitumen (i.a. roofing material) (NMD ID 16) 5 90 5 0
copper (i.a. sheets, pipes) (NMD ID 41) 5 0 95 0
elastomeres (i.a. epdm, roofing, foils) (NMD ID 20) 10 85 5 0
EoL electronics - passive components 5 35 60 0
finishes (adhered to wood, plastic, metal) (NMD ID 2) 0 100 0 0
Galvanised steel (i.a. profiles, sheets) (NMD ID 75) 5 0 95 0
Metals, mixed (via residue (NMD ID 49) 5 5 90 0
no waste (empty scenario) (NMD ID 26) 0 0 0 0
plastics, reinforced (i.a. profiles, sheets, pipes) (NMD 0
0 100 0
ID 46)
plastics, via residue (NMD ID 43) 20 80 0 0
polyolefines (i.a. pe,pp) (i.a. pipes, foils) (NMD ID 57) 10 85 5 0
PVC, pipes (NMD ID 64) 10 20 70 0
Sewage, to wastewater treatment, Average (EU) 0 0 100 0
Steel, light (NMD ID 73) 1 0 87 12
Waste scenario for chromium steel (based on NMD 0
5 5 90
ID 50)
wood 'clean', via residue (NMD ID 35) | (u=10%) corr. 0
10 85 5
acc. EN16449
wood, contaminated (i.a. painted, preserved) (NMD 0
5 95 0
ID 36) | (u=10%, glue=2%) corr. acc. EN16449
Zinc / zinc coating galvanised steel (i.a. profiles, 0
5 0 95
sheets, zinc coating) (NMD ID 75)
Vaillant – aroTHERM plus 5 kW & uniTOWER plus | Page 14
5. LCA: Results
The following tables show the results of the indicators of the impact assessment, the resource input
as well as the waste materials and other output-flows. The results shown here refer to the declared
unit.
Table 13: Overview of the considered information modules showing all phases of the building life cycle accor-
ding to EN 15804 (X = module declared; MND = module not declared)
Bene-
fits
and
loads
be-
Construc-
Production phase Use phase End-of-life phase yond
tion phase
the
sys-
tem
bound
ary
s s e
-n
e to
la ire ta my lp wp au Rs tro p s n a rT g n iru tc a fu n a M tro p s n a rT
c o rp
n
o ita lla ts n I/ n o itc u rts n o C e s U e c n a n e tn ia M ria p e R s tn e m e c a lp e R la w e n e R e s u y g re n e la n o ita re p O e s u re ta w la n o ita re p O
n
o
itilo
m e d n o itc u rts n eo Dc - tro p s n a rT g n is s e c o rp e ts a W la s o p s iD
p g yn
reil
vc
o ey scc uee eRR R -- ,, la it
A1 A2 A3 A4 A5 B1 B2 B3 B4 B5 B6 B7 C1 C2 C3 C4 D
X X X X X X X X X X X X X X X X X
Vaillant – aroTHERM plus 5 kW & uniTOWER plus | Page 15
Table 14: Results of the LCA – Environmental impact indicators: aroTHERM plus 5 kW & uniTOWER plus
Indicator
(Impact Unit A1 A2 A3 A4 A5 B1 B2 B3 B4 B5 B6 B7 C1 C2 C3 C4 D
Category)
mol H+
AP 1,00E+01 7,82E-01 6,83E-01 1,80E-01 3,75E-01 0,00E+00 1,08E-03 0,00E+00 0,00E+00 0,00E+00 6,23E+01 0,00E+00 0,00E+00 1,30E-02 3,66E-02 9,49E-04 -2,34E+00
eqv.
GWP-to- kg CO2
1,04E+03 1,24E+02 4,23E+01 3,10E+01 1,10E+02 5,40E-01 1,84E-01 0,00E+00 0,00E+00 0,00E+00 1,10E+04 0,00E+00 0,00E+00 2,25E+00 8,90E+01 6,77E-01 -3,32E+02
tal eqv.
kg CO2
GWP-b 4,52E+00 5,51E-02 -5,53E+01 1,43E-02 5,52E+01 0,00E+00 1,87E-04 0,00E+00 0,00E+00 0,00E+00 3,20E+02 0,00E+00 0,00E+00 1,04E-03 3,79E-01 4,59E-02 9,92E-01
eqv.
kg CO2
GWP-f 1,03E+03 1,23E+02 9,75E+01 3,10E+01 5,49E+01 5,40E-01 1,84E-01 0,00E+00 0,00E+00 0,00E+00 1,07E+04 0,00E+00 0,00E+00 2,25E+00 8,86E+01 6,31E-01 -3,33E+02
eqv.
GWP-lu- kg CO2
1,43E+00 4,60E-02 1,49E-01 1,14E-02 5,06E-02 0,00E+00 5,38E-05 0,00E+00 0,00E+00 0,00E+00 2,48E+01 0,00E+00 0,00E+00 8,24E-04 5,09E-03 4,81E-05 -9,35E-02
luc eqv.
ETP-fw CTUe 9,07E+04 1,65E+03 4,03E+03 4,17E+02 3,14E+03 0,00E+00 6,50E+00 0,00E+00 0,00E+00 0,00E+00 1,50E+05 0,00E+00 0,00E+00 3,02E+01 6,59E+02 1,78E+02 -2,65E+04
disease
PM 7,76E-05 1,10E-05 7,78E-06 2,79E-06 3,22E-06 0,00E+00 1,02E-08 0,00E+00 0,00E+00 0,00E+00 1,63E-04 0,00E+00 0,00E+00 2,02E-07 3,30E-07 1,80E-08 -2,32E-05
incidence
EP-m kg N eqv. 1,26E+00 2,67E-01 1,29E-01 6,34E-02 6,05E-02 0,00E+00 2,25E-04 0,00E+00 0,00E+00 0,00E+00 7,90E+00 0,00E+00 0,00E+00 4,59E-03 9,56E-03 5,51E-04 -3,46E-01
kg PO4
EP-fw 1,11E-01 1,23E-03 6,35E-03 3,13E-04 3,66E-03 0,00E+00 1,39E-06 0,00E+00 0,00E+00 0,00E+00 1,14E+00 0,00E+00 0,00E+00 2,27E-05 2,16E-04 1,90E-06 -1,78E-02
eqv.
mol N
EP-T 1,63E+01 2,94E+00 1,52E+00 6,99E-01 7,44E-01 0,00E+00 2,43E-03 0,00E+00 0,00E+00 0,00E+00 9,74E+01 0,00E+00 0,00E+00 5,06E-02 1,07E-01 3,54E-03 -4,38E+00
eqv.
HTP-c CTUh 5,34E-06 5,42E-08 1,99E-07 1,35E-08 2,90E-07 0,00E+00 6,57E-11 0,00E+00 0,00E+00 0,00E+00 3,88E-06 0,00E+00 0,00E+00 9,81E-10 4,66E-08 1,01E-10 -1,56E-06
HTP-nc CTUh 9,81E-05 1,80E-06 5,64E-06 4,56E-07 3,28E-06 0,00E+00 3,17E-09 0,00E+00 0,00E+00 0,00E+00 1,32E-04 0,00E+00 0,00E+00 3,31E-08 4,30E-07 6,23E-09 2,03E-06
kBq U235
IR 4,06E+01 7,78E+00 4,89E+00 1,96E+00 1,77E+00 0,00E+00 6,64E-03 0,00E+00 0,00E+00 0,00E+00 1,90E+03 0,00E+00 0,00E+00 1,42E-01 2,33E-01 1,17E-02 -1,29E+00
eqv.
SQP Pt 4,96E+03 1,59E+03 9,05E+03 4,06E+02 4,99E+02 0,00E+00 1,48E+00 0,00E+00 0,00E+00 0,00E+00 5,36E+04 0,00E+00 0,00E+00 2,94E+01 3,17E+01 6,15E+00 -3,36E+03
kg CFC 11
ODP 6,74E-05 2,72E-05 1,02E-05 6,85E-06 4,02E-06 0,00E+00 2,35E-08 0,00E+00 0,00E+00 0,00E+00 8,99E-04 0,00E+00 0,00E+00 4,96E-07 1,60E-06 3,46E-08 -1,62E-05
eqv.
kg
POCP NMVOC 5,15E+00 8,35E-01 4,55E-01 2,00E-01 2,27E-01 0,00E+00 9,68E-04 0,00E+00 0,00E+00 0,00E+00 2,47E+01 0,00E+00 0,00E+00 1,45E-02 2,84E-02 1,14E-03 -1,73E+00
eqv.
ADP-f MJ 1,34E+04 1,86E+03 1,57E+03 4,68E+02 5,49E+02 0,00E+00 1,13E+01 0,00E+00 0,00E+00 0,00E+00 2,20E+05 0,00E+00 0,00E+00 3,39E+01 5,69E+01 2,65E+00 -3,22E+03
ADP-mm kg Sb-eqv. 3,80E-01 3,08E-03 1,59E-02 7,86E-04 1,21E-02 0,00E+00 2,49E-06 0,00E+00 0,00E+00 0,00E+00 7,76E-02 0,00E+00 0,00E+00 5,70E-05 1,06E-04 1,04E-06 -1,09E-01
m3 world
WDP 3,51E+02 6,58E+00 3,15E+01 1,67E+00 1,27E+01 0,00E+00 6,90E-03 0,00E+00 0,00E+00 0,00E+00 2,46E+03 0,00E+00 0,00E+00 1,21E-01 2,44E+00 6,40E-02 -5,44E+01
eqv.
AP = Acidification; GWP-total = Global warming potential – Total; GWP-b = Global warming potential – Biogenic; GWP-f = Global warming potential – Fossil; GWP-luluc = Global warming potential - Land use and land use change; ETP-fw
= Ecotoxicity, freshwater; PM = Particulate Matter; EP-m = Eutrophication marine; EP-fw = Eutrophication, freshwater; EP-t = Eutrophication, terrestrial; HTP-c = Human toxicity, cancer; HTP-nc = Human toxicity, non-cancer; IR =
Ionising radia-tion, human health; SQP = Land use; ODP = Ozone depletion; POCP = Photochemical ozone formation - human health; ADP-f = Resource use, fossils; ADP-mm = Resource use, minerals and metals; WDP = Water use
Vaillant – aroTHERM plus 5 kW & uniTOWER plus | Page 16
Table 15: Results of the LCA – Resource consumption, output streams & waste categories: aroTHERM plus 5 kW & uniTOWER plus
Parame-
Unit A1 A2 A3 A4 A5 B1 B2 B3 B4 B5 B6 B7 C1 C2 C3 C4 D
ter
PERE MJ 1,49E+03 2,31E+01 8,10E+02 5,86E+00 7,17E+01 0,00E+00 3,02E-02 0,00E+00 0,00E+00 0,00E+00 4,16E+04 0,00E+00 0,00E+00 4,24E-01 5,64E+00 9,92E-02 -7,83E+02
PERM MJ 3,42E+00 0,00E+00 4,73E+02 0,00E+00 1,43E+01 0,00E+00 0,00E+00 0,00E+00 0,00E+00 0,00E+00 0,00E+00 0,00E+00 0,00E+00 0,00E+00 0,00E+00 0,00E+00 0,00E+00
PERT MJ 1,49E+03 2,31E+01 1,28E+03 5,86E+00 8,60E+01 0,00E+00 3,02E-02 0,00E+00 0,00E+00 0,00E+00 4,16E+04 0,00E+00 0,00E+00 4,24E-01 5,82E+00 1,00E-01 -7,83E+02
PENRE MJ 1,33E+04 1,97E+03 1,46E+03 4,97E+02 5,52E+02 0,00E+00 1,25E+01 0,00E+00 0,00E+00 0,00E+00 2,30E+05 0,00E+00 0,00E+00 3,60E+01 5,86E+01 2,77E+00 -3,41E+03
PENRM MJ 8,78E+02 0,00E+00 2,23E+02 0,00E+00 3,30E+01 0,00E+00 0,00E+00 0,00E+00 0,00E+00 0,00E+00 0,00E+00 0,00E+00 0,00E+00 0,00E+00 0,00E+00 0,00E+00 -1,35E+01
PENRT MJ 1,42E+04 1,97E+03 1,68E+03 4,97E+02 5,85E+02 0,00E+00 1,25E+01 0,00E+00 0,00E+00 0,00E+00 2,30E+05 0,00E+00 0,00E+00 3,60E+01 6,07E+01 2,82E+00 -3,43E+03
SM kg 7,93E+01 0,00E+00 3,98E+00 0,00E+00 2,50E+00 0,00E+00 0,00E+00 0,00E+00 0,00E+00 0,00E+00 0,00E+00 0,00E+00 0,00E+00 0,00E+00 0,00E+00 0,00E+00 1,26E-01
RSF MJ 0,00E+00 0,00E+00 0,00E+00 0,00E+00 0,00E+00 0,00E+00 0,00E+00 0,00E+00 0,00E+00 0,00E+00 0,00E+00 0,00E+00 0,00E+00 0,00E+00 0,00E+00 0,00E+00 0,00E+00
NRSF MJ 0,00E+00 0,00E+00 0,00E+00 0,00E+00 0,00E+00 0,00E+00 0,00E+00 0,00E+00 0,00E+00 0,00E+00 0,00E+00 0,00E+00 0,00E+00 0,00E+00 0,00E+00 0,00E+00 0,00E+00
FW m3 1,11E+01 2,24E-01 9,17E-01 5,70E-02 4,10E-01 0,00E+00 2,52E-04 0,00E+00 0,00E+00 0,00E+00 1,84E+02 0,00E+00 0,00E+00 4,13E-03 8,80E-02 2,98E-03 -1,35E+00
HWD kg 1,20E-01 4,65E-03 1,19E-02 1,19E-03 5,82E-03 0,00E+00 1,60E-05 0,00E+00 0,00E+00 0,00E+00 1,46E-01 0,00E+00 0,00E+00 8,59E-05 5,63E-02 3,58E-06 3,20E-02
NHWD kg 3,15E+02 1,16E+02 3,61E+01 2,97E+01 1,96E+01 0,00E+00 9,32E-02 0,00E+00 0,00E+00 0,00E+00 7,43E+02 0,00E+00 0,00E+00 2,15E+00 2,20E+00 1,09E+01 -1,17E+02
RWD kg 3,60E-02 1,22E-02 5,52E-03 3,07E-03 1,84E-03 0,00E+00 1,00E-05 0,00E+00 0,00E+00 0,00E+00 1,56E+00 0,00E+00 0,00E+00 2,23E-04 2,22E-04 1,64E-05 -2,96E-03
CRU kg 0,00E+00 0,00E+00 6,82E-01 0,00E+00 4,30E-01 0,00E+00 0,00E+00 0,00E+00 0,00E+00 0,00E+00 0,00E+00 0,00E+00 0,00E+00 0,00E+00 1,36E+01 0,00E+00 0,00E+00
MFR kg 0,00E+00 0,00E+00 1,02E+01 0,00E+00 6,68E+00 0,00E+00 0,00E+00 0,00E+00 0,00E+00 0,00E+00 0,00E+00 0,00E+00 0,00E+00 0,00E+00 2,04E+02 0,00E+00 0,00E+00
MER kg 0,00E+00 0,00E+00 0,00E+00 0,00E+00 0,00E+00 0,00E+00 0,00E+00 0,00E+00 0,00E+00 0,00E+00 0,00E+00 0,00E+00 0,00E+00 0,00E+00 0,00E+00 0,00E+00 0,00E+00
EE-total MJ 0,00E+00 0,00E+00 1,91E+01 0,00E+00 0,00E+00 0,00E+00 0,00E+00 0,00E+00 0,00E+00 0,00E+00 0,00E+00 0,00E+00 0,00E+00 0,00E+00 0,00E+00 0,00E+00 6,92E+02
EET MJ 0,00E+00 0,00E+00 1,21E+01 0,00E+00 0,00E+00 0,00E+00 0,00E+00 0,00E+00 0,00E+00 0,00E+00 0,00E+00 0,00E+00 0,00E+00 0,00E+00 0,00E+00 0,00E+00 4,38E+02
EEE MJ 0,00E+00 0,00E+00 7,02E+00 0,00E+00 0,00E+00 0,00E+00 0,00E+00 0,00E+00 0,00E+00 0,00E+00 0,00E+00 0,00E+00 0,00E+00 0,00E+00 0,00E+00 0,00E+00 2,54E+02
PERE = Renewable primary energy ex. raw materials; PERM = Renewable primary energy used as raw materials; PERT = Renewable primary energy total; PENRE = Non-renewable primary energy ex. raw materials; PENRM = Non-
renewable primary energy used as raw materials; PENRT = Non-renewable primary energy total; SM = Use of secondary material; RSF = use of renewable secondary fuels; NRSF = Use of non-renewable secondary fuels; FW = Use of net
fresh water; HWD = Hazardous waste disposed; NHWD = Non-hazardous waste disposed; RWD = Radioactive waste disposed; CRU = Components for re-use; MFR = Materials for recycling; MER = Materials for energy recovery; EE-total
= Exported energy, total; EET = Exported energy thermic; EEE = Exported energy electric
Vaillant – aroTHERM plus 5 kW & uniTOWER plus | Page 17
6. LCA: Interpretation
For an easier understanding, the results are processed graphically, in order to recognize relationships
and connections between the data more clearly.
The following figure shows the percentage of the product phases in the environmental impact catego-
ries.
WDP
ADP-mm
ADP-f
POCP
ODP
SQP
IR
HTP-nc
HTP-c
EP-T
EP-fw
EP-m
PM
ETP-fw
GWP-luluc
GWP-f
GWP-b
GWP-total
AP
-20% 0% 20% 40% 60% 80% 100%
A1 A2 A3 A4 A5 B1 B2 B3 B4 B5 B6 B7 C1 C2 C3 C4 D
Figure 5: Percentage of the product phases in the environmental impact categories of aroTHERM plus 5 kW &
uniTOWER plus
As can be seen in the graph, the operational energy use (module B6) dominates in almost all environ-
mental impact categories, followed by the raw material supply (module A1). Furthermore, for the be-
nefits or loads outside the system boundaries (module D) the benefits (negative values) dominate over
the loads (positive values) in most of the environmental impact categories.
The limitations regarding the interpretation of the results are due to the assumptions made for the
LCA, because it assesses the real world in a simplified model. It can be assumed that the results for the
declared products are representative, because the quality of the data used can be classified as good
overall. All relevant process-specific data could be collected in the operational data collection. Consi-
stent data sets from the Ecoinvent database were available for all inputs and outputs.
As the raw material supply (module A1) has a big impact on the results for all products, the used data-
sets from Ecoinvent 3.6 for the different materials are important. For all materials matching datasets
were found, thus, a high data quality can be assumed.
Vaillant – aroTHERM plus 5 kW & uniTOWER plus | Page 18
7. References
DIN EN ISO 14040 DIN EN ISO 14040: 2009-11: Environmental management - Life cycle assess-
ment - Principles and framework (ISO 14040:2006)
DIN EN ISO 14044 DIN EN ISO 14044: 2018-05: Environmental management - Life cycle assess-
ment - Requirements and guidelines (ISO 14044:2006 + Amd 1:2017)
DIN EN ISO 15804 DIN EN ISO 15804:2014-07: Sustainability of construction works - Environmen-
tal product declarations - Core rules for the product category of construction.
Ecoinvent, 2019 Ecoinvent database version 3.6 (2019)
EN ISO 14025 EN ISO 14025:2010: Environmental labels and declarations - Type III environ-
mental declarations - Principles and procedures (ISO 14025:2006)
Huber, 2022 Temperature Control; Blog powered by Huber Kältemaschinenbau AG;
http://www.temperaturecontrol.blog/sustainable-environmentally-safe-and-
future-proof-temperature-control
PCR A General Product Category Rules for Construction Products from the EPD pro-
gram of Kiwa-Ecobility Experts; Version 2.1
PCR B PCR Guidance-Texts for Building-Related Products and Services: From the
range of Environmental Product Declarations of Institute Construction and En-
vironment e.V. (IBU) – Part B: Requirements on the EPD for HVAC Appliances
R<THiNK, 2023 R<THiNK: EPD & LCA tool by NIBE (2023)
PCR EPDItaly019 EPDItaly Core PCR - HVAC Home Appliances, GPI version 5.0 (2021)
www.epditaly.it
CPC 43912 PCR 2021:02 'Air-conditioning machines product group classification: UN CPC
43912' version 1.0.
EU regulation Implementing Directive 2009/125/EC of the European Parliament and of the
206/212 Council with regard to ecodesign requirements for air conditioners and com-
fort fans.
EU regulation of the Commission dated 18 February 2013 supplementing Guideline 2010/30
811/2013 /EU of the European Parliament and Council with regard to energy marking of
room heaters, combination heating appliances, integrated systems comprising
room heaters, temperature controllers and solar equipment as well as inte-
grated systems comprising combination heating appliances, temperature con-
trollers and solar equipment.
EU regulation of the Commission dated 11 July 2014 supplementing Directive 2010/30/EU
1254/2014 of the European Parliament and of the Council with regard to energy labelling
of residential ventilation units
IPCC, 2007 Climate Change 2007: Synthesis Report. Contribution of Working Groups I, II
and III to the Fourth Assessment Report of the Intergovernmental Panel on
Climate Change [Core Writing Team, Pachauri, R.K and Reisinger, A. (eds.)].
IPCC, Geneva, Switzerland, 104 pp.
ISO 817 ISO 817:2014-05: Refrigerants - Designation and safety classification, Beuth-
Verlag, Berlin.
Vaillant – aroTHERM plus 5 kW & uniTOWER plus | Page 19
DIN EN 14825 DIN EN 14825:2019-07: Air conditioners, liquid chilling packages and heat
pumps, with electrically driven compressors, for space heating and cooling -
Testing and rating at part load conditions and calculation of seasonal perfor-
mance; German version EN 14825:2018, Beuth-Verlag, Berlin.
DIN EN 13141 DIN EN 13141-11:2019-04: Ventilation for buildings - Performance testing of
components/products for residential ventilation - Part 1: Externally and inter-
nally mounted air transfer devices; German version EN 13141-1:2019, Beuth-
Verlag, Berlin.
PSR-0013 PSR-0013-ed2.0-EN-2019-12-06: Specific rules for thermodynamic generators
PEP ecopassport with electric compression for heating and/or cooling of premises and/or the
production of domestic hot water. PCR part B, v. 1.2: Requirements on the EPD
for Air conditioner; Heat generators; Volume flow controllers and volume flow
limiters for ventilation systems.
ISO 15686 ISO 15686-1:2011-05: Buildings and constructed assets - Service life planning
- Part 1: General principles and framework.
Vaillant – aroTHERM plus 5 kW & uniTOWER plus | Page 20
Publisher:
Kiwa-Ecobility Experts Mail DE.Ecobility.Experts@kiwa.com
Kiwa GmbH, Ecobility Experts Web www.kiwa.com/de/en/themes/
Wattstraße 11-13 ecobility-experts/
13355 Berlin
Germany
Programme operator:
Kiwa-Ecobility Experts Mail DE.Ecobility.Experts@kiwa.com
Kiwa GmbH, Ecobility Experts Web www.kiwa.com/de/en/themes/
Wattstraße 11-13 ecobility-experts/
13355 Berlin
Germany
LCA practitioner:
Kiwa GmbH, Ecobility Experts Tel +49 30 46 77 61 52
Wattstraße 11-13 Mail DE.Nachhaltigkeit@kiwa.com
13355 Berlin Web www.kiwa.com
Germany
Owner of the declaration:
Vaillant GmbH Tel +49 2191 57 67 920
Berghauser Straße 40 Mail service@heizungonline.de
42859 Remscheid Web www.vaillant.de
Germany
Kiwa-Ecobility Experts is
established member of the
Vaillant – aroTHERM plus 5 kW & uniTOWER plus | Page 21
