ENVIRONMENTAL PRODUCT DECLARATION
as per ISO 14025 and EN 15804+A2
Owner of the Declaration dormakaba International Holding GmbH
Publisher Institut Bauen und Umwelt e.V. (IBU)
Programme holder Institut Bauen und Umwelt e.V. (IBU)
Declaration number EPD-DOR-20220358-CBA4-EN
Issue date 15.03.2023
Valid to 14.03.2028
Automatic Sliding Door ST FLEX
dormakaba
www.ibu-epd.com | https://epd-online.com
General Information
dormakaba Automatic Sliding Door ST FLEX
Programme holder Owner of the declaration
IBU – Institut Bauen und Umwelt e.V. dormakaba International Holding GmbH
Hegelplatz 1 DORMA Platz 1
10117 Berlin 58256 Ennepetal
Germany Germany
Declaration number Declared product / declared unit
EPD-DOR-20220358-CBA4-EN The declared unit is one piece (1 pc.) of the ST FLEX automatic sliding
door system without drive comprising:
• ST FLEX sliding panels,
• ST FLEX side screens and
• product packaging
This declaration is based on the product category rules: Scope:
Automatic doors, automatic gates, and revolving door systems, This EPD refers to the entire life cycle of a specific ST FLEX automatic
01.08.2021 sliding door system. The production location is dormakaba
(PCR checked and approved by the SVR) Zusmarshausen, Germany. Green electricity is used at the production
facility. The material and energy flows were taken into consideration
accordingly.
Issue date
The year of data collection is 2022.
15.03.2023
The owner of the declaration shall be liable for the underlying information
and evidence; the IBU shall not be liable with respect to manufacturer
information, life cycle assessment data and evidences.
Valid to
14.03.2028 The EPD was created according to the specifications of EN 15804+A2. In
the following, the standard will be simplified as EN 15804.
Verification
The standard EN 15804 serves as the core PCR
Independent verification of the declaration and data according to ISO
14025:2011
internally X externally
Dipl.-Ing. Hans Peters
(Chairman of Institut Bauen und Umwelt e.V.)
Florian Pronold Dr.-Ing. Wolfram Trinius,
(Managing Director Institut Bauen und Umwelt e.V.) (Independent verifier)
1 Environmental Product Declaration - dormakaba - Automatic Sliding Door ST FLEX
Product
seals and top and bottom seals
Product description/Product definition • Flexible and adaptable to project requirements
ST FLEX stands for an automatic sliding door system
manufactured by dormakaba. The automatic sliding door Base materials/Ancillary materials
system comprises a sliding door operator including sensors and Performance data of the product with respect to its
control unit. It can be opened on one or two sides and characteristics in accordance with the relevant technical
configured with or without side screens. provision which can be applied are mentioned above.
Thanks to its low profile width, the ST FLEX automatic sliding The ST FLEX Automatic Sliding Door comprises the following
door is extremely versatile and allows plenty of light components including packaging:
penetration. With its various designs, it is the perfect solution
for sophisticated projects.
To meet all requirements the ST FLEX system can be
combined with different ES operator versions, among others ES
PROLINE and ES 200. For placing the ST FLEX on the market
the following legal provisions apply:
• EN 16005
• DIN 18650-1/ -2
• ISO 13849-1
• EN 60335-1
• EN 60335-2-103
• IEC 60335-2-103
• 2011/65/EU ROHS3 Directive
Application
The product contains partial articles which contain
The ST Flex is an elegant solution for all passage areas. The
substances listed in the Candidate List of REACH
slender profile system provides visual openness and stability in
Regulation 1907/2006/EC (date: 17.01.2023)
various configurations. On request, the automatic sliding door
exceeding 0.1 percentage by mass: no
systems from dormakaba are manufactured for individual
dimensions of various building projects. Details regarding
The Candidate List can be found on the ECHA website
different operator systems that can be combined with the ST
address: https://echa.europa.eu/de/home.
FLEX profile system are available in the respective product
catalogues. Reference service life
The reference serivce life of the Automatic Sliding Door ST Flex
Technical Data
amountsd to 10 years, depending on the application and
• Low profile width frequency of use. For repairs and renewals, suitable spare
• Attractive glass surfaces thanks to slender frames parts are available. The ST Flex is testes and certified to EN
• High stability and torsional rigidity 16005, meaning they are designed to withstand a minimum of
• Low k-value of frame due to double glazing 1.000.000 cycles.
• Excellent insulation features thanks to interlocking side
LCA: Calculation rules
Declared Unit
The declared unit is 1 piece of the product: Automatic Sliding Construction stage - Modules A4-A5
Door ST FLEX The construction process stage includes:
Name Value Unit — A4, transport to the building site;
Declared unit 1 pce. — A5, installation into the building;
including provision of all materials, products and
Mass (total system) 252.73 kg
energy, as well as waste processing up to the end-of
waste state or disposal of final residues during the
System boundary
construction process stage.
The type of EPD is: cradle-to-gate with options,
modules C1–C4, and module D (A1–A3 + C + D and
additional modules: A4 + A5 + B6)
Use stage - Module B6
The use stage related to the operation of the building
Production - Module A1-A3
includes:
The product stage includes:
— B6, operational energy use
— A1, raw material extraction, processing and
mechanical treatments, processing of secondary
material input (e.g. recycling processes),
End-of-life stage– Modules C1-C4 and D
— A2, transport to the manufacturer,
The end-of-life stage includes:
— A3, manufacturing and assembly including provision
— C1, de-construction, demolition:
of all materials, products and energy, as well as waste
— C2, transport to waste processing;
processing up to the end-of waste state.
— C3, waste processing for reuse, recovery and/or
2 Environmental Product Declaration - dormakaba - Automatic Sliding Door ST FLEX
recycling; manufactured, used or handled at the end of the product´s
— C4, disposal; lifespan: Global
including provision and all transport, provision of all
materials, products and related energy and water use.
Comparability
Module D (Benefits and loads beyond the system
boundary) includes: Basically, a comparison or an evaluation of EPD data is only
— D, recycling potentials, expressed as net impacts possible if all the data sets to be compared were created
and benefits. according to EN 15804 and the building context, respectively
the product-specific characteristics of performance, are taken
Geographic Representativeness into account. Background database: GaBi, SP40.
Land or region, in which the declared product system is
LCA: Scenarios and additional technical information
End of life (C1-C4)
Characteristic product properties of biogenic carbon
C1: The product expansion depends on the building. The
Information on describing the biogenic Carbon Content at product share is so low that no environmental burden is
factury gate assumed.
Name ValueUnit C2: Transport to waste treatment at end of life is 50km.
Biogenic carbon content in accompanying kg Name Value Unit
0.003
packaging C Collected separately waste type waste type 244 kg
Reuse - kg
The following technical scenario information is required for the Recycling 34.8 kg
declared modules.
Energy recovery 8.51 kg
Transport to the building site (A4) Landfilling 200 kg
Name Value Unit Transport to waste management 50 km
Litres of fuel (per 1 kg) 0.00276 l/100km
The product is disassembled in a recycling process. Material
Transport distance via medium truck 100 km recycling is then assumed for the metals, electronics and
Capacity utilisation (including empty runs) 55 % electromechanics. The plastic components are assumed to be
incinerated with energy recovery. Glass and minor proportions
Transport distance is declared for a distance of 100km by truck
of residues arising from the recycling process are landfilled.
in order to allow scaling to a specific point of installation.
Region for the End of Life is: Global.
Installation into the building (A5)
Name Value Unit
Waste packaging (paper and plastic) 9 kg
3 Environmental Product Declaration - dormakaba - Automatic Sliding Door ST FLEX
LCA: Results
DESCRIPTION OF THE SYSTEM BOUNDARY (X = INCLUDED IN LCA; MND = MODULE OR INDICATOR NOT DECLARED; MNR
= MODULE NOT RELEVANT)
Benefits and
Construction loads beyond
Product stage Use stage End of life stage
process stage the system
boundaries
la ire ta m w a Ry lp p u s tro p s n a rT g n iru tc a fu n a M e h t m o rf tro p s n a rTe tis e h t o t e ta g y lb m e s s A e s U e c n a n e tn ia M ria p e R tn e m e c a lp e R tn e m h s ib ru fe R y g re n e la n o ita re p Oe s u re ta w la n o ita re p Oe s u n o itc u rts n o c -e Dn o itilo m e d tro p s n a rT g n is s e c o rp e ts a W la s o p s iD -e s u e R-y re v o c e R-g n ilc y c e Rla itn e to p
A1 A2 A3 A4 A5 B1 B2 B3 B4 B5 B6 B7 C1 C2 C3 C4 D
X X X X X MND MND MNR MNR MNR MND MND X X X X X
RESULTS OF THE LCA - ENVIRONMENTAL IMPACT according to EN 15804+A2: 1 piece Automatic Sliding Door ST FLEX
Parameter Unit A1-A3 A4 A5 C1 C2 C3 C4 D
GWP-total kg CO 2 eq 4.54E+02 2.21E+00 2.29E+01 0 1.07E+00 2.17E+01 3.06E+00 -7.14E+01
GWP-fossil kg CO 2 eq 4.52E+02 2.11E+00 2.29E+01 0 1.02E+00 2.16E+01 3.04E+00 -7.12E+01
GWP-biogenic kg CO 2 eq 1.54E+00 9.8E-02 5.33E-04 0 4.7E-02 1.3E-02 1E-02 -1.2E-01
GWP-luluc kg CO 2 eq 1.91E-01 5.03E-05 1E-03 0 2.43E-05 1E-03 9E-03 -3.9E-02
ODP kg CFC11 eq 2.45E-10 2.23E-16 1.15E-14 0 1.08E-16 1.09E-14 1.13E-14 -3.04E-10
AP mol H+ eq 2.95E+00 2E-03 4E-03 0 1E-03 4E-03 2.2E-02 -2.21E-01
EP-freshwater kg P eq 4.16E-04 4.52E-07 1.84E-06 0 2.18E-07 1.74E-06 5.22E-06 -5.32E-05
EP-marine kg N eq 6.48E-01 6.73E-04 9.18E-04 0 3.24E-04 8.69E-04 6E-03 -3.4E-02
EP-terrestrial mol N eq 7.39E+00 7E-03 1.9E-02 0 4E-03 1.8E-02 6.2E-02 -3.68E-01
kg NMVOC
POCP 1.41E+00 2E-03 3E-03 0 9.17E-04 2E-03 1.7E-02 -1.05E-01
eq
ADPE kg Sb eq 7.62E-04 6.34E-08 1.58E-07 0 3.06E-08 1.5E-07 2.73E-07 -3.71E-04
ADPF MJ 6.73E+03 3E+01 1.06E+01 0 1.44E+01 1E+01 3.99E+01 -1.04E+03
m3 world eq
WDP 3.14E+01 4E-03 2.34E+00 0 2E-03 2.21E+00 3.19E-01 -7.95E+00
deprived
GWP = Global warming potential; ODP = Depletion potential of the stratospheric ozone layer; AP = Acidification potential of land and water; EP =
Eutrophication potential; POCP = Formation potential of tropospheric ozone photochemical oxidants; ADPE = Abiotic depletion potential for non-fossil
resources; ADPF = Abiotic depletion potential for fossil resources; WDP = Water (user) deprivation potential)
RESULTS OF THE LCA - INDICATORS TO DESCRIBE RESOURCE USE according to EN 15804+A2: 1 piece Automatic Sliding
Door ST FLEX
Parameter Unit A1-A3 A4 A5 C1 C2 C3 C4 D
PERE MJ 7.3E+02 9.4E-02 2.76E+00 0 4.6E-02 2.69E+00 5.22E+00 -3.53E+02
PERM MJ 8.4E-02 0 0 0 0 -8.4E-02 0 0
PERT MJ 7.3E+02 9.4E-02 2.76E+00 0 4.6E-02 2.61E+00 5.22E+00 -3.53E+02
PENRE MJ 6.07E+03 3E+01 3.98E+02 0 1.45E+01 2.85E+02 3.99E+01 -1.04E+03
PENRM MJ 6.62E+02 0 -3.87E+02 0 0 -2.75E+02 0 0
PENRT MJ 6.73E+03 3E+01 1.06E+01 0 1.45E+01 1E+01 3.99E+01 -1.04E+03
SM kg 2.59E+01 0 0 0 0 0 0 0
RSF MJ 0 0 0 0 0 0 0 0
NRSF MJ 0 0 0 0 0 0 0 0
FW m3 1.75E+00 1.7E-04 5.6E-02 0 8.17E-05 5.3E-02 1E-02 -6.98E-01
PERE = Use of renewable primary energy excluding renewable primary energy resources used as raw materials; PERM = Use of renewable primary
energy resources used as raw materials; PERT = Total use of renewable primary energy resources; PENRE = Use of non-renewable primary energy
excluding non-renewable primary energy resources used as raw materials; PENRM = Use of non-renewable primary energy resources used as raw
materials; PENRT = Total use of non-renewable primary energy resources; SM = Use of secondary material; RSF = Use of renewable secondary fuels;
NRSF = Use of non-renewable secondary fuels; FW = Use of net fresh water
RESULTS OF THE LCA – WASTE CATEGORIES AND OUTPUT FLOWS according to EN 15804+A2:
1 piece Automatic Sliding Door ST FLEX
Parameter Unit A1-A3 A4 A5 C1 C2 C3 C4 D
HWD kg 1.04E-05 2.91E-09 4.04E-08 0 1.4E-09 3.82E-08 6.08E-07 -3.39E-06
NHWD kg 5.74E+01 3E-03 2.38E+00 0 1E-03 2.25E+00 2.01E+02 -1.1E+01
RWD kg 1.41E-01 3.22E-05 3.94E-04 0 1.55E-05 3.72E-04 4.54E-04 -8.6E-02
CRU kg 0 0 0 0 0 0 0 0
MFR kg 0 0 0 0 0 1.02E+01 0 0
MER kg 0 0 0 0 0 0 0 0
EEE MJ 0 0 4.24E+01 0 0 0 0 0
EET MJ 0 0 9.73E+01 0 0 0 0 0
4 Environmental Product Declaration - dormakaba - Automatic Sliding Door ST FLEX
HWD = Hazardous waste disposed; NHWD = Non-hazardous waste disposed; RWD = Radioactive waste disposed; CRU = Components for re-use;
MFR = Materials for recycling; MER = Materials for energy recovery; EEE = Exported electrical energy; EET = Exported thermal energy
RESULTS OF THE LCA – additional impact categories according to EN 15804+A2-optional:
1 piece Automatic Sliding Door ST FLEX
Parameter Unit A1-A3 A4 A5 C1 C2 C3 C4 D
Disease
PM 1.93E-05 1.11E-08 5.2E-08 0 5.36E-09 4.92E-08 2.7E-07 -3.54E-06
incidence
IR kBq U235 eq 2.32E+01 5E-03 3.5E-02 0 2E-03 3.4E-02 4.7E-02 -1.63E+01
ETP-fw CTUe 7.48E+03 2.12E+01 3.98E+00 0 1.02E+01 3.77E+00 2.28E+01 -3.38E+02
HTP-c CTUh 3.34E-06 4E-10 3.45E-10 0 1.93E-10 3.26E-10 3.38E-09 -3.37E-08
HTP-nc CTUh 4.38E-06 1.71E-08 3.49E-08 0 8.24E-09 3.3E-08 3.72E-07 -4.67E-07
SQP SQP 3.89E+02 7.7E-02 3.18E+00 0 3.7E-02 3.01E+00 8.31E+00 -8.33E+01
PM = Potential incidence of disease due to PM emissions; IR = Potential Human exposure efficiency relative to U235; ETP-fw = Potential comparative
Toxic Unit for ecosystems; HTP-c = Potential comparative Toxic Unit for humans (cancerogenic); HTP-nc = Potential comparative Toxic Unit for humans
(not cancerogenic); SQP = Potential soil quality index
Disclaimer 1 – for the indicator “Potential Human exposure efficiency relative to U235”. This impact category deals mainly with the
eventual impact of low-dose ionizing radiation on human health of the nuclear fuel cycle. It does not consider effects due to possible
nuclear accidents, occupational exposure or radioactive waste disposal in underground facilities. Potential ionizing radiation from the
soil, radon and from some construction materials is also not measured by this indicator.
Disclaimer 2 – for the indicators “abiotic depletion potential for non-fossil resources”, “abiotic depletion potential for fossil resources”,
“water (user) deprivation potential, deprivation-weighted water consumption”, “potential comparative toxic unit for ecosystems”,
“potential comparative toxic unit for humans – cancerogenic”, “Potential comparative toxic unit for humans - not cancerogenic”,
“potential soil quality index”. The results of this environmental impact indicator shall be used with care as the uncertainties on these
results are high as there is limited experience with the indicator.
References
Standards
DIN 18650-1 Further References
DIN 18650-1: 2010-06, Powered pedestrian doors –Part 1:
Product requirements and test methods. European Chemicals Agency (ECHA)
https:echa.europa.eu/de/home
DIN 18650-2
DIN 18650-2:2010-06, Powered pedestrian doors –Part 2: GaBi ts software
Safety at powered pedestrian doors. Sphera Solutions GmbH Gabi Software System and Database
for Life Cycle Engineering 1992-2020 Version 10.0.0.71
EN 15804 University of Stuttgart Leinfelden-Echterdingen
EN 15804:2012-04, Sustainability of construction works –
Environmental product declarations – Core rules for the product GaBi ts documentation
category of construction products; German version EN GaBi life cycle inventory data documentation
15804:2012. (https://www.gabisoftware.com/support/gabi/gabidatabase-
2020-lci-documentation/).
EN 16005
EN 16005:2013-01, Power operated pedestrian doorsets - IBU 2021
Safety in use - Requirements and test methods; German General Instructions for the EPD programme of Institut Bauen
version EN 16005:2012 und Umwelt e.V. Version 2.0, Berlin: Institut Bauen und Umwelt
e.V., 2021. www.ibu-epd.com
EN 60335-1
EN 60335-1; VDE 0700-1:2012-10:2012-10, Household and LCA-tool dormakaba
similar electrical appliances – Safety - Part 1: General LCA tool, ENS doors LCA tool no.: BU-DOR-202107-LT1-EN
requirements (IEC 60335-1:2010, modified); German version Developed by Sphera Solutions GmbH.
EN 60335-1:2012.
PCR Part A
EN 60335 PCR – Part A: Calculation Rules for the Life Cycle Assessment
EN 60335-2-103/A1; Household and similar electrical and Requirements on the Project Re-port according to EN
appliances - Safety - Part 2-103: Particularrequirements for 15804+A2:2019, Version 1.0, Institut Bauen und Umwelt e.V.,
drives for gates, doors and windows (IEC 61/2863/CDV:2005); www.ibu-epd.com.
German version EN 60335-2-103:2003/prA1:2005.2011/65/EU
PCR Part B
ISO 13849-1 PCR – Part B: Requirements on the EPD for Automatic doors,
ISO 13849-1:2008-12, Safety of machinery – Safetyrelated automatic gates, and revolving door systems, 08/2021, Institut
parts of control systems – Part 1: General principles for design Bauen und Umwelt e.V., www.ibu-epd.com
(ISO 13849-1:2006.)
REACH Regulation
ISO 14025 REACH Regulation (EC) No 1907/2006 of the European
DIN EN ISO 14025:201110, Environmental labels and Parliament and of the Council on the Registration, Evaluation,
declarations — Type III environmental declarations — Authorisation and Restriction of Chemicals.
Principles and procedures
5 Environmental Product Declaration - dormakaba - Automatic Sliding Door ST FLEX
ROHS3 Directive hazardous substances in electrical and electronic equipment
Directive 2011/65/EU of the European Parliament and of the
Council of 8 June 2011 on the restriction of the use of certain
6 Environmental Product Declaration - dormakaba - Automatic Sliding Door ST FLEX
Publisher
Institut Bauen und Umwelt e.V. +49 (0)30 3087748- 0
Hegelplatz 1 info@ibu-epd.com
10117 Berlin www.ibu-epd.com
Germany
Programme holder
Institut Bauen und Umwelt e.V. +49 (0)30 3087748- 0
Hegelplatz 1 info@ibu-epd.com
10117 Berlin www.ibu-epd.com
Germany
Author of the Life Cycle Assessment
dormakaba International Holding GmbH +49 2333 793-0
DORMA Platz 1 info.de@dormakaba.com
58256 Ennepetal www.dormakaba.com
Germany
Owner of the Declaration
dormakaba International Holding GmbH +49 2333 793-0
DORMA Platz 1 info.de@dormakaba.com
58256 Ennepetal www.dormakaba.com
Germany
7 Environmental Product Declaration - dormakaba - Automatic Sliding Door ST FLEX
