ENVIRONMENTAL PRODUCT DECLARATION
as per ISO 14025 and EN 15804+A2
Owner of the Declaration Türk Ytong A.S.
Publisher Institut Bauen und Umwelt e.V. (IBU)
Programme holder Institut Bauen und Umwelt e.V. (IBU)
Declaration number EPD-TYS-20220218-CCB1-EN
Issue date 19.07.2023
Valid to 18.07.2028
Autoclaved Aerated Concrete Reinforced Panel
Türk Ytong Sanayi A.Ş
www.ibu-epd.com | https://epd-online.com
General Information
Türk Ytong Sanayi A.Ş Autoclaved Aerated Concrete Reinforced Panel
Programme holder Owner of the declaration
IBU – Institut Bauen und Umwelt e.V. Türk Ytong A.S.
Hegelplatz 1 Aydinevler Mahallesi, Inönü Caddesi, Gökçe Sokak Maltepe No:3
10117 Berlin 34854 Istanbul
Germany Turkey
Declaration number Declared product / declared unit
EPD-TYS-20220218-CCB1-EN 1 m3 Autoclaved Aerated Concrete Reinforced Panel with an average
density of 575.3 kg/m3
This declaration is based on the product category rules: Scope:
Aerated concrete, 01.08.2021 The EPD is performed for an Autoclaved Aerated Concrete Reinforced
(PCR checked and approved by the SVR) Panel manufactured by Türk Ytong Sanayi A.Ş at two production plants
located in Dilovası and Antalya in Türkiye. The data is representative for
the year 2020.
Issue date The owner of the declaration shall be liable for the underlying information
and evidence; the IBU shall not be liable with respect to manufacturer
19.07.2023
information, life cycle assessment data and evidences.
The EPD was created according to the specifications of EN 15804+A2. In
Valid to
the following, the standard will be simplified as EN 15804.
18.07.2028
Verification
The standard EN 15804 serves as the core PCR
Independent verification of the declaration and data according to ISO
14025:2011
internally X externally
Dipl.-Ing. Hans Peters
(Chairman of Institut Bauen und Umwelt e.V.)
Florian Pronold Dr. Matthew Fishwick,
(Managing Director Institut Bauen und Umwelt e.V.) (Independent verifier)
1 Environmental Product Declaration - Türk Ytong Sanayi A.Ş - Autoclaved Aerated Concrete Reinforced Panel
Product
Name Value Unit
Product description/Product definition
Water 40-50 %
The product investigated in this EPD is an Autoclaved Aerated
Silica Sand 25-35 %
Concrete Reinforced Panel. Autoclaved aerated concrete is
classified as a porous, steam-cured lightweight concrete. The Cement 7-14 %
product is also known as a Ytong Panel. Lime 5-10 %
Steel 2-5 %
Ytong Panels are large-sized building elements containing
Gypsum 1-3 %
double rows of steel reinforcement, produced in various
Kaolin 1-2 %
thicknesses and up to 600 cm in length. Ytong panels can be
produced in 10, 12.5, 15-30 cm thicknesses; 400, 500, and 600 *Others 0-1 %
cm in lengths with a standard width of 60 cm. They are used for
completion of walls, roofs, and floors in large square meter Cement: Portland cement is used in the production of
buildings such as housing projects, hotels, shopping malls, autoclaved aerated concrete reinforced panels. Portland
educational, cultural, sports and industrial buildings. For the cement is produced according to EN 197-1. The cement in the
placing on the market of the product in the European mixture serves as a binding agent.
Union/European Free Trade Association (EU/EFTA) (with the Lime: The lime used in the AAC production is obtained by
exception of Switzerland) Regulation (EU) No. 305/2011 (CPR) burning natural limestone which serves as a
applies. The product needs a declaration of performance taking binder.
into consideration EN 12602:2016 - Prefabricated reinforced Steel Reinforcement: Since the product is reinforced AAC,
components of autoclaved aerated concrete - specification and double rows of steel reinforcement are placed inside the cake
the CE-marking. For the application and use the respective during production.
national provisions apply. Water: Throughout the production, water and water vapour are
used for different processes.
Application
Gypsum: The gypsum used in the product which comes from
Ytong Autoclaved Aerated Concrete (AAC) Reinforced Panel is
natural sources, helps to reduce the setting time, and increase
used in many areas such as warehouses, factories, shopping
the strength of the product.
malls, office spaces etc. It is produced with double row steel
*Others: Some minor additives such as kaolin, aluminium
reinforcement and applied with dry mounting technique, for
powders/pastes, and anticorrosive agents are used during
example:
production.
• Horizontal wall panels; external and internal walls, fire
walls. No substances included in the Candidate List of Substances of
• Vertical wall panels; external and internal walls, fire Very High Concern for authorization under the REACH
walls. regulations are present in this product either above the
• Load-Bearing wall panels; load bearing walls of panel threshold for registration with the European Chemicals Agency
system buildings, load bearing fire walls. or above 0.1% (wt/wt).
• Roof panels; building roofs
• Floor panels; building floors Manufacturing
• Lintels; door and window openings in external and The ground quartz sand is mixed with the other raw materials
internal walls. with the addition of water and aluminium powder/paste in a
mixer and poured into moulds. The lime is slaked by water
Technical Data
exothermically.
Technical properties of the Autoclaved Aerated Concrete The aluminum reacts in an alkaline environment, thus gaseous
Reinforced Panel are provided in the below table. hydrogen is formed, which fills the pores of the mass. The
Technical Properties pores usually have a diameter of 0.5 – 1.5 mm and are filled
with air. After setting, the semi-solid cake, is cut into a final
Name Value Unit
dimension with high accuracy.
Compressive strength 2 - 6 N/mm2
The steel reinforcement is manufactured in the plant. The
Gross density 350 - 600 kg/m3 reinforcement elements are installed in the moulds after the
Tensile strength 0.4 - 1 N/mm2 anti-corrosion treatment.
The formation of the final properties of the components takes
Modulus of elasticity 1000 - 2250 N/mm2
place during the subsequent steam curing for 6-12 hours at
Thermal conductivity 0.09 - 0.16 W/(mK) around 190°C and a pressure of approx. 12 bar in steam
Water vapour diffusion resistance factor 0.5 - pressure boilers, the so-called autoclaves. The substances
Moisture content at 23 °C, 80% <4 M.-% turned into calcium silicate hydrates like those found in nature,
correspond to the mineraltobermorite.
Bending strength (longitudinal) 0.4 - 1 N/mm2
The steam is released back into the system after the
Shrinkage <0.2 mm/m
completion of the curing process to condensate for further
Performance data of the product in accordance with the autoclave cycles. The resulting condensate is called process
declaration of performance with respect to its essential water. In this way, energy is saved and there is no waste water
characteristics according to EN 12602:2016 - Prefabricated during the production process.
reinforced components of autoclaved aerated concrete.
Packaging
Base materials/Ancillary materials A wooden pallet and a steel wire are used as packaging
The main materials used in the product are listed below in materials.
terms of mass percentages.
Environment and health during use
2 Environmental Product Declaration - Türk Ytong Sanayi A.Ş - Autoclaved Aerated Concrete Reinforced Panel
When the products are used as designated and according to
the current state of knowledge, there are no hazards to water, Reference service life
air and soil. When used normally and in accordance with the A 50 year reference service life is considered.
designated purpose, no health risks or restrictions are to be
anticipated.
LCA: Calculation rules
Dimova, S. in 2018 and published by the publication's office of
Declared Unit the European Union.
The declared unit is 1 m3 of Autoclaved Aerated Concrete
Reinforced Panel with an average density of 575.3 kg/m3. C2: Transport to EoL
A 100 km distance is assumed as the transport distance of the
Declared unit
waste product to the waste processing area.
Name Value Unit
Declared unit 1 m3 C3: Waste processing for reuse, recovery or recycling
Gross density 575.3 kg/m3
This module is considered zero since there is no need for the
The product investigated is an average product. Türk Ytong
after-life processes of the product.
produces AAC wall panels between 350 - 600 kg/m3.
C4: Disposal
System boundary
It is estimated that the amount of steel reinforcement used in
System boundary of this EPD is cradle to grave with module D
the product is recycled whereas the rest is landfilled. This
(A + B + C + D).
means that around 98 % of the product is landfilled and the rest
is recycled.
A1: Raw Material Supply
This stage considers the impact of raw materials used in the
D: Benefits
product. These raw materials are lime, Portland cement,
Following a conservative approach, it is assumed that the scrap
gypsum, silica sand, kaolin, paraffin, reinforcement steel and
will follow electric arc furnace (EAF) route. Thus, no benefit is
aluminium powder.
allocated at this stage.
A2: Transport to manufacturer Geographic Representativeness
The transport routes and distances are calculated from Land or region, in which the declared product system is
supplier-specific information. manufactured, used or handled at the end of the product´s
lifespan: Global
A3: Manufacturing
The manufacturing stage includes the following processes.
Comparability
• Mixing of ground quartz with other raw materials with
Basically, a comparison or an evaluation of EPD data is only
the addition of water and aluminium powder.
possible if all the data sets to be compared were created
• Pouring of the slurry into moulds.
according to EN 15804 and the building context, respectively
• Slaking of lime by water exothermically.
the product-specific characteristics of performance, are taken
• Formation of gaseous hydrogen which fills the pores of
into account.
the mass.
• Final sizing, shaping and cutting of AAC wall panels.
Cut-Off Criteria
• Preparation of steel reinforcement.
A 1% cut-off was applied. Data for elementary flows to and from
• Installation of steel reinforcement in the molds.
the product system contributing to a minimum of 99% of the
• Steam curing process for 6-12 hours at around 190°C
declared environmental impacts have been included.
and a pressure of approx. 12 bar in steam pressure
boilers, so-called autoclaves.
Allocations
• Releasing of steam after completion of the curing
Water consumption, energy consumption and raw material
process for further cycles.Condensation of water which
transportation were weighted according to 2020 production
will be used for further productions.
volumes. In addition, hazardous and non-hazardous waste
A4: Transportation to building site
amounts were also allocated from the 2020 total waste
Transport of the final product to the customers is taken as the
generation.
weighted average values for transport to customers in 2020.
LCA Modelling, Calculation and Data Quality
A5: Installation into building
The results of the LCA with the indicators as per EPD
The use of cement mortar and additional steel reinforcement
requirements are given in the LCA result tables. Life cycle
during the installation is considered in this stage.
impacts were calculated using the EN15804+A2 method
implementation which has an aligned methodology based on
B1: Use/Application
EF 3.0 method. For resource use calculations (PERE, PERM,
CO absorption of AAC wall panel during its service life is
2
PERT, PENRE, PENRT), {CED LHV}, (Cumulative Energy
calculated in this module.
Demand) – Lower Heating Values) method which is prepared
by PRé consultants is used. The mandatory indicators
C1: Deconstruction/Demolition
according to EN15804+A2 are declared for the EPD. The
It is assumed that 0.239 MJ energy is needed for the
characterization methodology referenced in the EN15804+A2 is
deconstruction/demolition of 1 kg of final product according to
used for the calculation.
JRC technical report called 'Model for Life Cycle Assessment
(LCA) of buildings' prepared by Dos Santos Gervasio, H. and
3 Environmental Product Declaration - Türk Ytong Sanayi A.Ş - Autoclaved Aerated Concrete Reinforced Panel
SimaPro 9.3 LCA software and the ecoinvent 3.8 LCA database Geographical Scope
were used to model the product life cycle. The geographical scope of this EPD for the manufacturing of
Country-specific electricity mix is used for electricity the declared product is Türkiye whereas the geographical
consumption. scope for the other modules is global.
LCA: Scenarios and additional technical information
amounts are displayed below for 1 m3 of AAC wall panel.
Characteristic product properties biogenic carbon
Name Value Unit
The raw material used in the product do not include biogenic
Other resources - Cement mortar 11.9 kg
carbon. For the packaging, the use of a wooden pallet
contributes to the biogenic carbon. However, since the total Other resources - Steel reinforcement 1.8 kg
mass of biogenic carbon containing materials is less than 5 %
According to the manufacturer, reference service life of the
of the total mass of the product and accompanying packaging,
product is 50 years.
the declaration of biogenic carbon content is omitted.
Reference service life
Scenario Information
Name Value Unit
Transport to the building site (A4)
Life Span according to the manufacturer 50 a
Relevant transport information of the final products to the
customers are provided in the below table. All the transport
End of life (C1-C4)
distances and routes are supplier-specific.
Considering common sector practices, the steel reinforcement
Name Value Unit
used in the product is recycled whereas the rest of the product
Transport distance - Average distance by truck 212 km is landfilled. Quantities displayed in below table is for 1 m3 of
Capacity utilisation (including empty runs) 100 % the final product.
Gross density of products transported 575.3kg/m3 Name Value Unit
Transport distance - Average distance by Collected as mixed construction waste 575.3 kg
910 km
container ship Landfilling 545.8 kg
Recycled 29.5 kg
Installation into the building (A5)
Energy recovery - kg
Impacts of using cement mortar and additional steel
reinforcement during the installation are considered. The
4 Environmental Product Declaration - Türk Ytong Sanayi A.Ş - Autoclaved Aerated Concrete Reinforced Panel
LCA: Results
Disclaimer:
EP-freshwater: This indicator has been calculated as 'kg P eq” as required in the characterization model (EUTREND model, Struijs et
al., 2009b, as implemented in ReCiPe; http://eplca.jrc.ec.europa.eu/LCDN/developerEF.xhtml)
DESCRIPTION OF THE SYSTEM BOUNDARY (X = INCLUDED IN LCA; ND = MODULE OR INDICATOR NOT DECLARED; MNR =
MODULE NOT RELEVANT)
Benefits and
Construction loads beyond
Product stage Use stage End of life stage
process stage the system
boundaries
la ire ta m w a Ry lp p u s tro p s n a rT g n iru tc a fu n a M e h t m o rf tro p s n a rTe tis e h t o t e ta g y lb m e s s A e s U e c n a n e tn ia M ria p e R tn e m e c a lp e R tn e m h s ib ru fe R y g re n e la n o ita re p Oe s u re ta w la n o ita re p Oe s u n o itc u rts n o c -e Dn o itilo m e d tro p s n a rT g n is s e c o rp e ts a W la s o p s iD -e s u e R-y re v o c e R-g n ilc y c e Rla itn e to p
A1 A2 A3 A4 A5 B1 B2 B3 B4 B5 B6 B7 C1 C2 C3 C4 D
X X X X X X MND MNR MNR MNR MND MND X X X X X
RESULTS OF THE LCA - ENVIRONMENTAL IMPACT according to EN 15804+A2: 1 m³ Ytong® Reinforced Autoclaved Aerated
Wall Panel with average density of 575.3 kg/m3
Parameter Unit A1 A2 A3 A4 A5 B1 C1 C2 C3 C4 D
GWP-total kg CO 2 eq 1.39E+02 1.47E+01 2.3E+01 4.31E+01 4.54E+00 -8.58E+01 2.44E+01 9.38E+00 0 5.83E+00 0
GWP-fossil kg CO 2 eq 1.37E+02 1.47E+01 2.26E+01 4.3E+01 4.4E+00 -8.58E+01 2.39E+01 9.37E+00 0 5.76E+00 0
GWP-
biogenic kg CO 2 eq 1.71E+00 1.24E-02 2.28E-01 2.87E-02 1.01E-01 0 2.44E-01 8.09E-03 0 5.88E-02 0
GWP-luluc kg CO 2 eq 5.41E-01 5.95E-03 1.61E-01 2E-02 2.34E-02 0 1.74E-01 3.75E-03 0 5.86E-03 0
ODP kg CFC11 eq 5.99E-06 3.39E-06 5.8E-07 9.68E-06 2.18E-07 0 5.61E-07 2.17E-06 0 1.75E-06 0
AP mol H+ eq 5.1E-01 4.66E-02 1.45E-01 3.76E-01 1.75E-02 0 1.57E-01 2.66E-02 0 4.87E-02 0
EP-
kg P eq 3.1E-02 9.55E-04 2.28E-02 2.54E-03 1.37E-03 0 2.47E-02 6.14E-04 0 1.67E-03 0
freshwater
EP-marine kg N eq 1.28E-01 9.59E-03 2.46E-02 8.84E-02 4.35E-03 0 2.64E-02 5.41E-03 0 1.68E-02 0
EP-terrestrial mol N eq 1.38E+00 1.05E-01 2.23E-01 9.78E-01 4.53E-02 0 2.39E-01 5.89E-02 0 1.83E-01 0
kg NMVOC
POCP 3.7E-01 3.86E-02 6.15E-02 2.8E-01 1.26E-02 0 6.57E-02 2.27E-02 0 5.28E-02 0
eq
ADPE kg Sb eq 9.8E+02 2.22E+02 2.45E+02 6.32E+02 3.68E+01 0 2.57E+02 1.42E+02 0 1.35E+02 0
ADPF MJ 6.37E-04 5.16E-05 3.26E-05 1.34E-04 2.37E-05 0 3.28E-05 3.32E-05 0 1.88E-05 0
m3 world eq
WDP 3.56E+03 6.72E-01 1.16E+03 1.78E+00 1.95E+00 0 8.74E+00 4.32E-01 0 5.9E+00 0
deprived
GWP = Global warming potential; ODP = Depletion potential of the stratospheric ozone layer; AP = Acidification potential of land and water; EP =
Eutrophication potential; POCP = Formation potential of tropospheric ozone photochemical oxidants; ADPE = Abiotic depletion potential for non-fossil
resources; ADPF = Abiotic depletion potential for fossil resources; WDP = Water (user) deprivation potential)
RESULTS OF THE LCA - INDICATORS TO DESCRIBE RESOURCE USE according to EN 15804+A2: 1 m³ Ytong® Reinforced
Autoclaved Aerated Wall Panel with average density of 575.3 kg/m3
Parameter Unit A1 A2 A3 A4 A5 B1 C1 C2 C3 C4 D
PERE MJ 9.69E+01 3.15E+00 5.13E+01 8.21E+00 5.37E+00 0 5.54E+01 2.03E+00 0 2.29E+00 0
PERM MJ 0 0 0 0 0 0 0 0 0 0 0
PERT MJ 9.69E+01 3.15E+00 5.13E+01 8.21E+00 5.37E+00 0 5.54E+01 2.03E+00 0 2.29E+00 0
PENRE MJ 9.82E+02 2.22E+02 2.45E+02 6.32E+02 3.68E+01 0 2.57E+02 1.42E+02 0 1.35E+02 0
PENRM MJ 0 0 0 0 0 0 0 0 0 0 0
PENRT MJ 9.82E+02 2.22E+02 2.45E+02 6.32E+02 3.68E+01 0 2.57E+02 1.42E+02 0 1.35E+02 0
SM kg 2.95E+01 0 0 0 0 0 0 0 0 0 0
RSF MJ 0 0 0 0 0 0 0 0 0 0 0
NRSF MJ 0 0 0 0 0 0 0 0 0 0 0
FW m3 6.64E+01 3.69E-02 2.09E+01 9.75E-02 7.57E-02 0 9.78E-02 2.38E-02 0 1.53E-01 0
PERE = Use of renewable primary energy excluding renewable primary energy resources used as raw materials; PERM = Use of renewable primary
energy resources used as raw materials; PERT = Total use of renewable primary energy resources; PENRE = Use of non-renewable primary energy
excluding non-renewable primary energy resources used as raw materials; PENRM = Use of non-renewable primary energy resources used as raw
materials; PENRT = Total use of non-renewable primary energy resources; SM = Use of secondary material; RSF = Use of renewable secondary fuels;
NRSF = Use of non-renewable secondary fuels; FW = Use of net fresh water
RESULTS OF THE LCA – WASTE CATEGORIES AND OUTPUT FLOWS according to EN 15804+A2:
1 m³ Ytong® Reinforced Autoclaved Aerated Wall Panel with average density of 575.3 kg/m3
Parameter Unit A1 A2 A3 A4 A5 B1 C1 C2 C3 C4 D
HWD kg 0 0 8.4E-01 0 0 0 0 0 0 0 0
NHWD kg 0 0 1.5E-01 0 0 0 0 0 0 0 0
5 Environmental Product Declaration - Türk Ytong Sanayi A.Ş - Autoclaved Aerated Concrete Reinforced Panel
RWD kg 0 0 0 0 0 0 0 0 0 0 0
CRU kg 0 0 0 0 0 0 0 0 0 0 0
MFR kg 0 0 0 0 0 0 0 0 0 0 0
MER kg 0 0 0 0 0 0 0 0 0 0 0
EEE MJ 0 0 0 0 0 0 0 0 0 0 0
EET MJ 0 0 0 0 0 0 0 0 0 0 0
HWD = Hazardous waste disposed; NHWD = Non-hazardous waste disposed; RWD = Radioactive waste disposed; CRU = Components for re-use;
MFR = Materials for recycling; MER = Materials for energy recovery; EEE = Exported electrical energy; EET = Exported thermal energy
RESULTS OF THE LCA – additional impact categories according to EN 15804+A2-optional:
1 m³ Ytong® Reinforced Autoclaved Aerated Wall Panel with average density of 575.3 kg/m3
Parameter Unit A1 A2 A3 A4 A5 B1 C1 C2 C3 C4 D
Disease
PM 6.58E-06 1.17E-06 6.37E-07 3.04E-06 2.59E-07 0 6.73E-07 7.55E-07 0 9.9E-07 0
incidence
IR kBq U235 eq 8.9E+00 1.14E+00 2.47E-01 3.19E+00 4E-01 0 2.06E-01 7.32E-01 0 6.32E-01 0
ETP-fw CTUe 2.26E+03 1.74E+02 2.37E+02 4.77E+02 8.85E+01 0 2.52E+02 1.11E+02 0 1.06E+02 0
HTP-c CTUh 9.17E-07 5.67E-09 1.09E-08 1.83E-08 5.2E-08 0 4.47E-09 3.59E-09 0 4.23E-09 0
HTP-nc CTUh 1.62E-06 1.75E-07 1.97E-07 4.58E-07 6.64E-08 0 2.05E-07 1.13E-07 0 6.51E-08 0
SQP SQP 1.13E+03 1.53E+02 2.17E+01 3.79E+02 4.44E+01 0 2.22E+01 9.9E+01 0 3.24E+02 0
PM = Potential incidence of disease due to PM emissions; IR = Potential Human exposure efficiency relative to U235; ETP-fw = Potential comparative
Toxic Unit for ecosystems; HTP-c = Potential comparative Toxic Unit for humans (cancerogenic); HTP-nc = Potential comparative Toxic Unit for humans
(not cancerogenic); SQP = Potential soil quality index
Disclaimer 1 – for the indicator “Potential Human exposure efficiency relative to U235”. This impact category deals mainly with the
eventual impact of low-dose ionizing radiation on human health of the nuclear fuel cycle. It does not consider effects due to possible
nuclear accidents, occupational exposure nor due to radioactive waste disposal in underground facilities. Potential ionizing radiation
from the soil, from radon and from some construction materials is also not measured by this indicator.
Disclaimer 2 – for the indicators “abiotic depletion potential for non-fossil resources”, “abiotic depletion potential for fossil resources”,
“water (user) deprivation potential, deprivation-weighted water consumption”, “potential comparative toxic unit for ecosystems”,
“potential comparative toxic unit for humans – cancerogenic”, “Potential comparative toxic unit for humans - not cancerogenic”,
“potential soil quality index”. The results of this environmental impact indicator shall be used with care as the uncertainties on these
results are high or as there is limited experienced with the indicator.
This EPD was created using a software tool.
References
EN 197-1 Characterisation factors, first edition.
EN 197-1:2011 Cement Part 1: Composition, specifications and
conformity criteria for common cements Institut Bauen und Umwelt
Institut Bauen und Umwelt e.V., Berlin(pub.): Generation of
EN 12602:2016 Environmental Product Declarations
Prefabricated reinforced components of autoclaved aerated (EPDs); www.ibu-epd.de
concrete
REACH
ISO 14025 Directive (EG) No. 1907/2006 of the European Parliament and
DIN EN ISO 14025:2011-10: Environmental labels and of the Council dated 18 December 2006 on the registration,
declarations — Type III environmental declarations — evaluation, approval and restriction of chemical substances
Principles and procedures (REACH), for establishing a European Agency for chemical
substances, for amending Directive 1999/45/EC and for
EN IS0 14040 annulment of Directive (EEC) No. 793/93 of the Council,
EN ISO 14044:2014 Environmental management - Life cycle Directive (EC) No. 1488/94 of the Commission, Guideline
assessment - Requirements and guidelines 76/769/EEC of the Council and Guidelines 91/155/EEC,
93/67/EEC, 93/105/EC and 2000/21/EC of the Commission
EN ISO 14044
EN ISO 14044:2014 Environmental management - Life cycle Regulation (EU) No 305/2011
assessment - Requirements and guidelines Regulation (EU) No 305/2011 of the European Parliament and
Of The Council of 9 March 2011 laying down harmonised
EN 15804 conditions for the marketing of construction products and
EN 15804:2012+A2:2019: Sustainability of construction works repealing Council Directive 89/106/EEC
— Environmental Product Declarations — Core rules for the
product category of construction product PCR Part A
Institut Bauen und Umwelt e.V., Berlin (pub.): Product Category
EUTREND Model Rules for Construction Products from the range of
Struijs, J., Beusen, A., van Jaarsveld, H. and Huijbregts, M.A.J. Environmental Product Declarations of Institut Bauen und
(2009b). Aquatic Eutrophication. Chapter 6 in: Goedkoop, M., Umwelt (IBU), Part A: Calculation Rules for the Life Cycle
Heijungs, R., Huijbregts, M.A.J., De Schryver, A., Struijs, J., Assessment and Requirements on the Background Report.
Van Zelm, R. (2009). ReCiPe 2008 A life cycle impact April 2013
assessment method which comprises harmonised category
indicators at the midpoint and the endpoint level. Report I:
6 Environmental Product Declaration - Türk Ytong Sanayi A.Ş - Autoclaved Aerated Concrete Reinforced Panel
PCR Part B Switzerland https://ecoinvent.org/
Part B: Requirements on the EPD for Aerated concrete, Version
1.5, Institut Bauen und Umwelt e.V., www.bau-umwelt.com, SimaPro
2017 SimaPro software for LCA calculations, developed by PRé
Sustainability, Stationsplein 121, 3818 LE Amersfoort,
Ecoinvent Netherlands, https://simapro.com
Ecoinvent dataset, developed by the Swiss Centre for Life
Cycle Inventories, Technoparkstrasse 1,8005 Zurich,
7 Environmental Product Declaration - Türk Ytong Sanayi A.Ş - Autoclaved Aerated Concrete Reinforced Panel
Publisher
Institut Bauen und Umwelt e.V. +49 (0)30 3087748- 0
Hegelplatz 1 info@ibu-epd.com
10117 Berlin www.ibu-epd.com
Germany
Programme holder
Institut Bauen und Umwelt e.V. +49 (0)30 3087748- 0
Hegelplatz 1 info@ibu-epd.com
10117 Berlin www.ibu-epd.com
Germany
Author of the Life Cycle Assessment
Metsims Sustainability Consulting +90 534 499 32 40
Elmas Studio Levent,Sultan Selim Mah. Lalegül Sok. info@metsims.com
No: 7/18 www.metsims.com
34415 4.Levent, Istanbul
Turkey
Owner of the Declaration
Türk Ytong A.S. + 90 216 396 66 00
Aydinevler Mahallesi, Inönü Caddesi, Gökçe Sokak ytong@ytong.com.tr
Maltepe No:3 www.ytong.com.tr
34854 Istanbul
Turkey
8 Environmental Product Declaration - Türk Ytong Sanayi A.Ş - Autoclaved Aerated Concrete Reinforced Panel
