Environmental product declaration
in accordance with ISO 14025 and EN 15804+A2
AXQJ-TT Pure TSLI 24kV AL 1x630/50mm² AFR
Owner of the declaration: Program operator:
Prysmian Group Norge AS The Norwegian EPD Foundation
Product: Declaration number:
AXQJ-TT Pure TSLI 24kV AL 1x630/50mm² AFR
NEPD-7468-6839-EN
Declared unit:
1 m Registration number:
This declaration is based on Product Category Rules: NEPD-7468-6839-EN
CEN Standard EN 15804:2012+A2:2019 serves as core
Issue date: 06.09.2024
PCR
The Norwegian EPD Foundation NPCR 027:2020 Part B for Electrical cables and wires Valid to: 06.09.2029
EPD software:
LCAno EPD generator ID: 532626
1 / 13
General information
Product Owner of the declaration:
AXQJ-TT Pure TSLI 24kV AL 1x630/50mm² AFR Prysmian Group Norge AS
Contact person: Anders Nymark
Phone: +47 90066733
e-mail: anders.nymark@prysmiangroup.com
Program operator: Manufacturer:
The Norwegian EPD Foundation Prysmian Group Norge AS
Post Box 5250 Majorstuen, 0303 Oslo, Norway Kjerraten 16
Phone: +47 977 22 020 3013 Drammen, Norway
web: www.epd-norge.no
Declaration number: Place of production:
Prysmian Group production site Nässjö (Sweden)
NEPD-7468-6839-EN
Vallgatan 5
571 41 Nässjö, Sweden
This declaration is based on Product Category Rules: Management system:
CEN Standard EN 15804:2012+A2:2019 serves as core PCR ISO 9001, ISO 14001, ISO 45001
NPCR 027:2020 Part B for Electrical cables and wires
Statement of liability: Organisation no:
The owner of the declaration shall be liable for the underlying 814 780 422
information and evidence. EPD Norway shall not be liable with respect
to manufacturer information, life cycle assessment data and
evidences.​
Declared unit: Issue date:
1 m AXQJ-TT Pure TSLI 24kV AL 1x630/50mm² AFR 06.09.2024
Declared unit with option: Valid to:
A1,A2,A3,A4,A5,B1,B2,B3,B4,B5,B6,B7,C1,C2,C3,C4,D 06.09.2029
Year of study:
2023
Functional unit: Comparability:
1 m of installed AXQJ-TT Pure TSLI 24 kV medium voltage single core EPD of construction products may not be comparable if they not
distribution cable, used to transmit a reference electric current of 1A comply with EN 15804 and seen in a building context.
over a 40 year lifetime, including waste treatment at end-of-life.
General information on verification of EPD from EPD tools: Development and verification of EPD:
Independent verification of data, other environmental information The declaration is created using EPD tool lca.tools ver EPD2022.03,
and the declaration according to ISO 14025:2010, § 8.1.3 and § 8.1.4. developed by LCA.no. The EPD tool is integrated in the company's
Verification of each EPD is made according to EPD-Norway’s management system, and has been approved by EPD Norway.
guidelines for verification and approval requiring that tools are i) Approval number: NEPDT33
integrated into the company's environmental management system, ii)
the procedures for use of the EPD tool are approved by EPD-Norway, Developer of EPD: Siri Andersen
and iii) the process is reviewed annually by an independent third
Reviewer of company-specific input data and EPD:​ Anders Nymark
party verifier. See Appendix G of EPD-Norway's General Programme
Instructions for further information on EPD tools
Verification of EPD tool: Approved:
Independent third party verification of the EPD tool, background data
and test-EPD in accordance with EPDNorway's procedures and
guidelines for verification and approval of EPD tools. Approval
number: NEPDT32.
Third party verifier:
Vito D’Incognito, Take Care International
(no signature required)
2 / 13
Product
Product description:
AXQJ-TT Pure TSLI 24KV AL
Halogen free and flame retardant on fire. Smoke generation at fire is small, low smoke density (makes evacuation easier) and is not harmful to
electrical equipment. Distribution cable for indoor use in 3-phase installation. Can be placed in pipes and in the ground.The cable is axially and
radially waterproof.
Product specification
Conductor material Aluminium
Conductor surface Bare
Longitudinal water blocking conductors Yes
Inner semi-conducting layer Yes
Core insulation material XLPE
Outer semi-conducting layer Yes
Drain wire Yes
Longitudinal water blocking cable Yes
Radial water blocking cable Yes
Screen construction Aluminium tape and copper wire
Screen Yes
Screen material Copper, bare
Concentric conductor Copper
Material inner sheath Other
Material outer sheath Halogenfree polymer
Laminated sheath Yes
Longitudinal water blocking screen Yes
Protective barrier Al/PE
Cable shape Round
Materials kg %
Adhesive 0,01 0,31
HFFR Polyolefin 0,61 22,03
Metal - Aluminium 1,12 40,84
Metal - Copper 0,28 10,12
Plastic - Polyethylene 0,72 26,07
Tape 0,02 0,63
Total 2,75 100,00
Technical data:
AXQJ-TT Pure TSLI 24KV AL 1X630/50mm² AFR
SAP code: 20217599
El nr. 1060213
STANDARDS APPLIED:
HD 620 Part 10, Section K and M, HD604 (halogen-free sheath) Design standard
IEC 60332-3-24 (Cat. C) Flame retardant
EN 60754-1 and EN 60754-2 Halogen free properties: EN 60754-1 (pH = 4,3, Conductivity = 10µS), EN
60754-2 ( < 0,5% Halogen)
Low smoke IEC 61034
Market:
Norway
Reference service life, product
40 years. Standard lifetime for energy distribution network applications, provided in appendix 1 of PSR for wires, cables, and accessories of PEP
Ecopassport.
Reference service life, building or construction works
40 years. Estimation made to match the product service life and keep the EPD environmental impact calculations at the product level.
LCA: Calculation rules
Declared unit:
1 m AXQJ-TT Pure TSLI 24kV AL 1x630/50mm² AFR
Cut-off criteria:
3 / 13
All major raw materials and all the essential energy is included. The production processes for raw materials and energy flows with very small
amounts (less than 1%) are not included. These cut-off criteria do not apply for hazardous materials and substances.
Allocation:
The allocation is made in accordance with the provisions of EN 15804. Incoming energy and water and waste production in-house is allocated
equally among all products through mass allocation. Effects of primary production of recycled materials is allocated to the main product in which
the material was used. The recycling process and transportation of the material is allocated to this analysis.
Data quality:
Specific data for the product composition are provided by the manufacturer. The data represent the production of the declared product and were
collected for EPD development in the year of study. Background data is based on EPDs according to EN 15804 and different LCA databases. The
data quality of the raw materials in A1 is presented in the table below.
Materials Source Data quality Year
Adhesive ecoinvent 3.6 Database 2019
HFFR Polyolefin ecoinvent 3.6 Database 2019
Metal - Aluminium ecoinvent 3.6 Database 2019
Metal - Copper ecoinvent 3.6 Database 2019
Plastic - Polyethylene ecoinvent 3.6 Database 2019
Tape ecoinvent 3.6 Database 2019
4 / 13
System boundaries (X=included, MND=module not declared, MNR=module not relevant)
Construction Beyond the system
Product stage Use stage End of life stage
installation stage boundaries
A1 A2 A3 A4 A5 B1 B2 B3 B4 B5 B6 B7 C1 C2 C3 C4 D
X X X X X X X X X X X X X X X X X
System boundary:
The flowchart below illustrates the system boundaries of the analysis:
Additional technical information:
APPLICATION PROPERTIES
Test voltage [kV] 50
Rated voltage U0/U (Um) 12/20 (24) kV
Halogen free acc. IEC/EN 60754-1/2
Max. conductor temperature [°C] 90
Min. outer temperature, fixed installation [°C] -60
Max. outer temperature, fixed installation [°C] 60
UV resistant Yes
Outdoor installation Yes
Min. outer temperature during installation [°C] -20
Max. outer temperature during installation [°C] 40
Underground installation Yes
Suitable as medium voltage cable Yes
Bending radius (rule) 15 x OD (cable overall diameter) during installation
10 x OD (cable overall diameter) fixed installed
8 x OD (cable overall diameter) when plowing down
waR slairetam tropsnarT gnirutcafunaM tropsnarT ylbmessA e​sU ecnanetniaM riapeR tnemecalpeR tnemhsibrufeR lanoitarepO ygrene esu lanoitarepO esu retaw -eD noitcurtsnoc noitilomed tropsnarT etsaW gnissecorp lasopsiD -yrevoceR-esueR laitnetop-gnilcyceR
5 / 13
LCA: Scenarios and additional technical information
The following information describe the scenarios in the different modules of the EPD.
Module A4 = In A4, a transport distance of 775 km from the Prysmian Group plant in Nässjö, Sweden to Loesmoen warehouse was included. A
distance of 300 km was then added as additional transport to market.
Modules A5 = 2 % product losses during installation are estimated by the company. No energy use for installation has been quantified since this
operation is assumed to be done with other products and should be assessed at a construction works level. Cable drums are reused and assumed
under the cut-off criterion of 1%.
Modules B1, B2, B3, B5, and B7 = Company data shows that no significant activities have been reported for use, maintenance, repair, replacement,
refurbishment, and water use. This reflects an absence of impacts during the 40 years reference service life of the cable in these modules.
Module B4 =
The service life of the building is the same as the service life of the product, no replacement activities are taking place in module B4
Module B6 = The operational energy use of the cable is calculated based on the methodology described in PEP Ecopassport, Product Specific Rules
(PSR) for wires, cables and accessories, reference PSR-0001-ed3-EN-2015 10 16. The following parameters are used to calculate the electricity loss
of the cable:
- Reference service life = 40 years (according to appendix 1 of the PSR)
- Number of conductors = 1 unit
- Use rate = 100% percent (according to appendix 1 of the PSR)
- Linear conductor resistivity = 0,0000469 Ohm per meter
- Current intensity = 1 Ampere
Module C1 = For both buildings and construction works, cables will be taken out as part of a larger demolition. The energy use for cable removal
compared to other heaver materials is assumed to be low. This module can therefore be included with zero impact.
Module C2 = 300 km is added as default transport in Norway to nearest waste treatment in C2.
Modules C3 and C4 = Waste treatment of the product follows the default values provided in EN 50693, Product Category Rules for life cycle
assessments of electronic and electrical products and systems, table G.4. This table specified how different types of raw materials used in A1 will
likely be treated during the end-of-life of the product. Waste treatments in C3 include material recycling and incineration with and without energy
recovery and fly ash extraction. Disposal in C4 consist of landfilling of different waste fractions and of ashes.
Module D = The recyclability of metals and plastics allows the producers a credit for the net scrap that is produced at the end of a product’s life.
The benefits from recycling of net scrap are described in formula from EN 15804:2012+A2:2019. Substitution of heat and electricity generated by
the incineration with energy recovery of plastic insulation and other parts is also calculated in module D.
Capacity utilisation Value
Transport from production place to user (A4) Distance (km) Fuel/Energy Consumption Unit
(incl. return) % (Liter/tonne)
Truck, over 32 tonnes, EURO 5 (km) 53,3 % 775 0,023 l/tkm 17,83
Assembly (A5) Unit Value
Product loss during installation (percentage of
Units/DU 0,02
cable)
Operational energy (B6) Unit Value
Electricity, Norway (kWh) kWh/DU 0,02
Capacity utilisation Value
Transport to waste processing (C2) Distance (km) Fuel/Energy Consumption Unit
(incl. return) % (Liter/tonne)
Truck, 16-32 tonnes, EURO 5 (km) 36,7 % 300 0,044 l/tkm 13,20
Waste processing (C3) Unit Value
Aluminium to recycling (kg) kg 0,79
Copper to recycling (kg) kg 0,17
Waste treatment of plastic mixture, incineration
kg 0,32
with energy recovery and fly ash extraction (kg)
Waste treatment of polyethylene (PE),
incineration with energy recovery and fly ash kg 0,36
extraction (kg)
Disposal (C4) Unit Value
Landfilling of aluminium (kg) kg 0,34
Landfilling of ashes from incineration of Plastic
kg 0,01
mixture, process per kg ashes and residues (kg)
Landfilling of ashes from incineration of
Polyethylene (PE), process per kg ashes and kg 0,01
residues (kg)
Landfilling of copper (kg) kg 0,11
Landfilling of plastic mixture (kg) kg 0,67
6 / 13
Benefits and loads beyond the system
boundaries (D) Unit Value
Substitution of electricity (MJ) MJ 1,18
Substitution of primary aluminium with net scrap
kg 0,60
(kg)
Substitution of primary copper with net scrap (kg) kg 0,02
Substitution of thermal energy, district heating
MJ 17,84
(MJ)
7 / 13
LCA: Results
The LCA results are presented below for the declared unit defined on page 2 of the EPD document.
Environmental impact
Indicator Unit A1 A2 A3 A4 A5 B1 B2 B3
GWP-total kg CO2 -eq 2,71E+01 4,72E-01 3,74E-01 2,42E-01 6,05E-01 0 0 0
GWP-fossil kg CO2 -eq 2,67E+01 4,71E-01 3,27E-01 2,42E-01 5,97E-01 0 0 0
GWP-biogenic kg CO2 -eq 2,22E-01 2,14E-04 3,77E-02 9,92E-05 5,19E-03 0 0 0
GWP-luluc kg CO2 -eq 1,44E-01 1,84E-04 9,41E-03 7,05E-05 3,08E-03 0 0 0
ODP kg CFC11 -eq 1,36E-06 1,02E-07 7,52E-08 5,58E-08 3,27E-08 0 0 0
AP mol H+ -eq 2,18E-01 3,90E-03 1,10E-03 1,02E-03 4,50E-03 0 0 0
EP-FreshWater kg P -eq 1,40E-03 4,27E-06 1,07E-05 1,84E-06 2,84E-05 0 0 0
EP-Marine kg N -eq 2,76E-02 1,26E-03 2,72E-04 3,05E-04 5,98E-04 0 0 0
EP-Terrestial mol N -eq 3,20E-01 1,39E-02 2,70E-03 3,38E-03 6,87E-03 0 0 0
POCP kg NMVOC -eq 9,65E-02 3,92E-03 6,50E-04 1,09E-03 2,07E-03 0 0 0
ADP-minerals&metals1 kg Sb-eq 9,46E-04 6,66E-06 6,09E-06 4,13E-06 1,94E-05 0 0 0
ADP-fossil1 MJ 3,31E+02 6,92E+00 1,72E+01 3,76E+00 7,24E+00 0 0 0
WDP1 m3 4,27E+03 5,13E+00 1,72E+03 2,88E+00 1,20E+02 0 0 0
Indicator Unit B4 B5 B6 B7 C1 C2 C3 C4 D
GWP-total kg CO2 -eq 0 0 4,00E-04 0 0 1,72E-01 1,83E+00 8,41E-02 -5,64E+00
GWP-fossil kg CO2 -eq 0 0 3,88E-04 0 0 1,72E-01 1,83E+00 8,41E-02 -5,51E+00
GWP-biogenic kg CO2 -eq 0 0 1,07E-05 0 0 6,99E-05 2,50E-05 7,24E-06 -2,51E-02
GWP-luluc kg CO2 -eq 0 0 1,60E-06 0 0 6,00E-05 4,31E-06 4,11E-06 -1,05E-01
ODP kg CFC11 -eq 0 0 2,70E-11 0 0 3,91E-08 2,45E-09 3,98E-09 -7,53E-03
AP mol H+ -eq 0 0 3,03E-06 0 0 7,01E-04 2,99E-04 1,05E-04 -4,63E-02
EP-FreshWater kg P -eq 0 0 2,79E-08 0 0 1,35E-06 2,27E-07 1,95E-07 -2,78E-04
EP-Marine kg N -eq 0 0 3,33E-07 0 0 2,08E-04 1,43E-04 1,17E-04 -5,23E-03
EP-Terrestial mol N -eq 0 0 4,33E-06 0 0 2,30E-03 1,50E-03 4,18E-04 -5,92E-02
POCP kg NMVOC -eq 0 0 1,17E-06 0 0 7,04E-04 3,62E-04 1,35E-04 -1,94E-02
ADP-minerals&metals1 kg Sb-eq 0 0 2,89E-08 0 0 4,65E-06 1,19E-07 1,04E-07 -4,42E-05
ADP-fossil1 MJ 0 0 5,29E-03 0 0 2,59E+00 1,73E-01 3,09E-01 -7,00E+01
WDP1 m3 0 0 9,22E-01 0 0 2,47E+00 9,01E-01 5,22E+00 -3,08E+03
GWP-total = Global Warming Potential total; GWP-fossil = Global Warming Potential fossil fuels; GWP-biogenic = Global Warming Potential biogenic; GWP-luluc =
Global Warming Potential land use and land use change; ODP = Depletion potential of the stratospheric ozone layer; AP = Acidification potential, Accumulated
Exceedance; EP-freshwater = Eutrophication potential, fraction of nutrients reaching freshwater end compartment: EP-marine = Eutrophication potential, fraction of
nutrients reaching marine end compartment; EP-terrestrial = Eutrophication potential, Accumulated Exceedance; POCP = Formation potential of tropospheric ozone;
ADP-minerals&metals = Abiotic depletion potential for non-fossil resources; ADP-fossil = Abiotic depletion for fossil resources potential; WDP = Water (user)
deprivation potential, deprivation-weighted water consumption
"Reading example: 9,0 E-03 = 9,0*10-3 = 0,009"
*INA Indicator Not Assessed
1. The results of this environmental impact indicator shall be used with care as the uncertainties on these results are high or as there is limited experienced with the
indicator
Remarks to environmental impacts
8 / 13
Additional environmental impact indicators
Indicator Unit A1 A2 A3 A4 A5 B1 B2 B3
PM Disease incidence 1,90E-06 3,98E-08 8,60E-09 2,13E-08 3,96E-08 0 0 0
IRP2 kgBq U235 -eq 7,67E-01 2,99E-02 5,81E-01 1,64E-02 2,82E-02 0 0 0
ETP-fw1 CTUe 1,39E+03 5,37E+00 1,02E+01 2,75E+00 3,37E+01 0 0 0
HTP-c1 CTUh 5,15E-08 0,00E+00 3,32E-10 0,00E+00 1,04E-09 0 0 0
HTP-nc1 CTUh 1,65E-06 5,59E-09 8,05E-09 2,66E-09 3,34E-08 0 0 0
SQP1 dimensionless 6,31E+01 6,41E+00 7,76E+00 4,31E+00 1,69E+00 0 0 0
Indicator Unit B4 B5 B6 B7 C1 C2 C3 C4 D
PM Disease incidence 0 0 2,20E-11 0 0 1,23E-08 1,25E-09 1,95E-09 -4,44E-07
IRP2 kgBq U235 -eq 0 0 9,60E-05 0 0 1,13E-02 3,78E-04 1,77E-03 -3,06E-01
ETP-fw1 CTUe 0 0 2,41E-02 0 0 1,91E+00 1,79E+00 2,77E+02 -1,73E+02
HTP-c1 CTUh 0 0 1,00E-12 0 0 0,00E+00 6,70E-11 1,60E-11 -1,49E-08
HTP-nc1 CTUh 0 0 2,70E-11 0 0 2,06E-09 2,88E-09 3,65E-10 -2,68E-07
SQP1 dimensionless 0 0 2,66E-03 0 0 1,78E+00 2,73E-02 8,61E-01 -1,15E+01
PM = Particulate Matter emissions; IRP = Ionizing radiation – human health; ETP-fw = Eco toxicity – freshwater; HTP-c = Human toxicity – cancer effects; HTP-nc =
Human toxicity – non cancer effects; SQP = Potential Soil Quality Index (dimensionless)
"Reading example: 9,0 E-03 = 9,0*10-3 = 0,009"
*INA Indicator Not Assessed
1. The results of this environmental impact indicator shall be used with care as the uncertainties on these results are high or as there is limited experienced with the
indicator
2. This impact category deals mainly with the eventual impact of low dose ionizing radiation on human health of the nuclear fuel cycle. It does not consider effects due
to possible nuclear accidents, occupational exposure nor due to radioactive waste disposal in underground facilities. Potential ionizing radiation from the soil, from
radon and from some construction materials is also not measured by this indicator.
9 / 13
Resource use
Indicator Unit A1 A2 A3 A4 A5 B1 B2 B3
PERE MJ 4,94E+01 1,10E-01 8,16E+00 4,73E-02 1,16E+00 0 0 0
PERM MJ 0,00E+00 0,00E+00 0,00E+00 0,00E+00 0,00E+00 0 0 0
PERT MJ 4,94E+01 1,10E-01 8,16E+00 4,73E-02 1,16E+00 0 0 0
PENRE MJ 2,92E+02 6,92E+00 1,72E+01 3,76E+00 6,45E+00 0 0 0
PENRM MJ 4,23E+01 0,00E+00 0,00E+00 0,00E+00 6,04E-02 0 0 0
PENRT MJ 3,34E+02 6,92E+00 1,72E+01 3,76E+00 6,51E+00 0 0 0
SM kg 2,40E-01 0,00E+00 0,00E+00 0,00E+00 4,80E-03 0 0 0
RSF MJ 3,96E-01 3,16E-03 3,20E-02 1,65E-03 8,70E-03 0 0 0
NRSF MJ 1,16E-01 1,69E-02 1,03E-01 5,55E-03 4,96E-03 0 0 0
FW m3 4,45E-01 8,58E-04 1,99E-02 4,28E-04 9,36E-03 0 0 0
Indicator Unit B4 B5 B6 B7 C1 C2 C3 C4 D
PERE MJ 0 0 6,85E-02 0 0 3,65E-02 7,79E-03 2,83E-02 -3,40E+01
PERM MJ 0 0 0,00E+00 0 0 0,00E+00 0,00E+00 0,00E+00 0,00E+00
PERT MJ 0 0 6,85E-02 0 0 3,65E-02 7,79E-03 2,83E-02 -3,40E+01
PENRE MJ 0 0 5,30E-03 0 0 2,59E+00 1,73E-01 3,09E-01 -7,00E+01
PENRM MJ 0 0 0,00E+00 0 0 0,00E+00 -3,93E+01 0,00E+00 0,00E+00
PENRT MJ 0 0 5,30E-03 0 0 2,59E+00 -3,92E+01 3,09E-01 -7,00E+01
SM kg 0 0 0,00E+00 0 0 0,00E+00 0,00E+00 0,00E+00 1,60E-02
RSF MJ 0 0 5,38E-05 0 0 1,31E-03 1,81E-04 5,88E-04 -1,01E-02
NRSF MJ 0 0 1,34E-04 0 0 4,66E-03 0,00E+00 1,56E-03 -5,02E-01
FW m3 0 0 5,12E-04 0 0 2,72E-04 1,07E-03 3,93E-04 -1,47E-01
PERE = Use of renewable primary energy excluding renewable primary energy resources used as raw materials; PERM = Use of renewable primary energy resources used
as raw materials; PERT = Total use of renewable primary energy resources; PENRE = Use of non renewable primary energy excluding non-renewable primary energy
resources used as raw materials; PENRM = Use of non renewable primary energy resources used as raw materials; PENRT = Total use of non renewable primary energy
resources; SM = Use of secondary materials; RSF = Use of renewable secondary fuels; NRSF = Use of non-renewable secondary fuels; FW = Net use of fresh water
"Reading example: 9,0 E-03 = 9,0*10-3 = 0,009"
*INA Indicator Not Assessed
10 / 13
End of life - Waste
Indicator Unit A1 A2 A3 A4 A5 B1 B2 B3
HWD kg 1,81E-01 4,32E-04 8,23E-02 2,06E-04 5,84E-03 0 0 0
NHWD kg 5,22E+00 4,26E-01 1,25E-01 3,27E-01 1,47E-01 0 0 0
RWD kg 7,45E-04 4,64E-05 2,56E-04 2,57E-05 2,19E-05 0 0 0
Indicator Unit B4 B5 B6 B7 C1 C2 C3 C4 D
HWD kg 0 0 3,40E-06 0 0 1,32E-04 0,00E+00 2,78E-02 2,19E-02
NHWD kg 0 0 4,08E-04 0 0 1,24E-01 0,00E+00 1,13E+00 -1,62E+00
RWD kg 0 0 4,74E-08 0 0 1,76E-05 0,00E+00 2,10E-06 -2,87E-04
HWD = Hazardous waste disposed; NHWD = Non-hazardous waste disposed; RWD = Radioactive waste disposed
"Reading example: 9,0 E-03 = 9,0*10-3 = 0,009"
*INA Indicator Not Assessed
End of life - Output flow
Indicator Unit A1 A2 A3 A4 A5 B1 B2 B3
CRU kg 0,00E+00 0,00E+00 0,00E+00 0,00E+00 0,00E+00 0 0 0
MFR kg 0,00E+00 0,00E+00 5,42E-03 0,00E+00 1,91E-02 0 0 0
MER kg 0,00E+00 0,00E+00 3,09E-01 0,00E+00 1,96E-02 0 0 0
EEE MJ 0,00E+00 0,00E+00 1,80E-01 0,00E+00 2,72E-02 0 0 0
EET MJ 0,00E+00 0,00E+00 2,72E+00 0,00E+00 4,11E-01 0 0 0
Indicator Unit B4 B5 B6 B7 C1 C2 C3 C4 D
CRU kg 0 0 0,00E+00 0 0 0,00E+00 0,00E+00 0,00E+00 0,00E+00
MFR kg 0 0 0,00E+00 0 0 0,00E+00 9,52E-01 6,04E-05 -6,26E-04
MER kg 0 0 0,00E+00 0 0 0,00E+00 6,74E-01 1,48E-06 -8,24E-05
EEE MJ 0 0 0,00E+00 0 0 0,00E+00 1,18E+00 9,59E-05 -2,02E-04
EET MJ 0 0 0,00E+00 0 0 0,00E+00 1,78E+01 1,45E-03 -3,06E-03
CRU = Components for re-use; MFR = Materials for recycling; MER = Materials for energy recovery; EEE = Exported energy electrical; EET = Exported energy thermal
"Reading example: 9,0 E-03 = 9,0*10-3 = 0,009"
*INA Indicator Not Assessed
Biogenic Carbon Content
Indicator Unit At the factory gate
Biogenic carbon content in product kg C 0,00E+00
Biogenic carbon content in accompanying packaging kg C 0,00E+00
Note: 1 kg biogenic carbon is equivalent to 44/12 kg CO2
11 / 13
Additional requirements
Greenhouse gas emissions from the use of electricity in the manufacturing phase
National production mix from import, low voltage (production of transmission lines, in addition to direct emissions and losses in grid) of applied
electricity for the manufacturing process (A3).
Electricity mix Source Amount Unit
Electricity, Sweden (kWh) ecoinvent 3.6 54,94 g CO2-eq/kWh
Dangerous substances
The product contains no substances given by the REACH Candidate list.
Indoor environment
Additional Environmental Information
Additional environmental impact indicators required in NPCR Part A for construction products
Indicator Unit A1 A2 A3 A4 A5 B1 B2 B3
GWPIOBC kg CO2 -eq 2,70E+01 4,72E-01 3,66E-01 2,42E-01 6,03E-01 0 0 0
Indicator Unit B4 B5 B6 B7 C1 C2 C3 C4 D
GWPIOBC kg CO2 -eq 0 0 3,99E-04 0 0 1,72E-01 1,83E+00 8,63E-02 -5,36E+00
GWP-IOBC: Global warming potential calculated according to the principle of instantaneous oxidation. In order to increase the transparency of biogenic carbon​
contribution to climate impact, the indicator GWP-IOBC is required as it declares climate impacts calculated according to the principle of instantaneous oxidation.​
GWP-IOBC is also referred to as GWP-GHG in context to Swedish public procurement legislation.
12 / 13
Bibliography
ISO 14025:2010. Environmental labels and declarations - Type III environmental declarations - Principles and procedures. International
Organization for Standardization.
ISO 14044:2006. Environmental management - Life cycle assessment - Requirements and guidelines. International Organization for
Standardization.
EN 15804:2012+A2:2019. Environmental product declaration - Core rules for the product category of construction products. European
Committee for Standardization.
ISO 21930:2017. Sustainability in buildings and civil engineering works - Core rules for environmental product declarations of construction
products. International Organization for Standardization.
EN 50693:2019. Product category rules for life cycle assessments of electronic and electrical products and systems. European Committee for
Standardization.
Ecoinvent v3, 2019. Allocation, cut-off by classification. Swiss Centre of Life Cycle Inventories.
Iversen et al., (2021). eEPD v2021.09, background information for EPD generator tool system verification, LCA.no. Report number: 07.21. System
verification report.
Philis et al., (2022). EPD generator for NPCR 027 part B for electrical wires and cables, background information for EPD generator application and
LCA data, LCA.no Report number: 03.22. PCR verification report.
EPD Norway (2022). NPCR Part A: Construction products and services. The Norwegian EPD foundation. Version 2.0 published 24.03.2021.
EPD Norway (2022). NPCR 027 Part B for electrical cables and wires. The Norwegian EPD foundation. Version 2.0 published 01.03.2022.
Program operator and publisher Phone: +47 977 22 020
The Norwegian EPD Foundation e-mail: post@epd-norge.no
Post Box 5250 Majorstuen, 0303 Oslo, Norway web: www.epd-norge.no
Owner of the declaration: Phone: +47 90066733
Prysmian Group Norge AS e-mail: anders.nymark@prysmiangroup.com
Kjerraten 16, 3013 Drammen web: www.prysmiangroup.no
Author of the Life Cycle Assessment Phone: +47 916 50 916
LCA.no AS e-mail: post@lca.no
Dokka 6A, 1671 Kråkerøy web: www.lca.no
Developer of EPD generator Phone: +47 916 50 916
LCA.no AS e-mail: post@lca.no
Dokka 6A, 1671 Kråkerøy web: www.lca.no
ECO Platform web: www.eco-platform.org
ECO Portal web: ECO Portal
13 / 13
