ENVIRONMENTAL PRODUCT DECLARATION
as per ISO 14025 and EN 15804+A2
Owner of the Declaration Hansgrohe Group
Publisher Institut Bauen und Umwelt e.V. (IBU)
Programme holder Institut Bauen und Umwelt e.V. (IBU)
Declaration number EPD-HAN-20220300-ICC2-EN
Issue date 24.02.2023
Valid to 23.02.2028
Basin Faucets
Hansgrohe Group
www.ibu-epd.com | https://epd-online.com
1. General Information
Hansgrohe Group Basin Faucets
Programme holder Owner of the declaration
IBU – Institut Bauen und Umwelt e.V. Hansgrohe Group
Hegelplatz 1 Auestr. 5-9
10117 Berlin 77761 Schiltach
Germany Germany
Declaration number Declared product / declared unit
EPD-HAN-20220300-ICC2-EN One (1) piece of an average basin faucet incl. packaging
This declaration is based on the product category rules: Scope:
Fittings and showers, 01.08.2021 This average EPD was determined on the basis of a weighted average of
(PCR checked and approved by the SVR) production volume from
2021 and relates to the plants in Offenburg and Schiltach, Germany,
Shanghai, China and Alpharetta, USA. This average EPD is valid for the
Issue date whole product group of chrome plated basin faucets. The EPD was formed
from >94% of the products involved in the sales quantity.
24.02.2023
The owner of the declaration shall be liable for the underlying information
and evidence; the IBU shall not be liable with respect to manufacturer
information, life cycle assessment data and evidences.
Valid to
23.02.2028 The EPD was created according to the specifications of EN 15804+A2. In
the following, the standard will be simplified as EN 15804.
Verification
The standard EN 15804 serves as the core PCR
Independent verification of the declaration and data according to ISO
14025:2011
internally X externally
Dipl.-Ing. Hans Peters
(Chairman of Institut Bauen und Umwelt e.V.)
Florian Pronold Dr Naeem Adibi,
(Managing Director Institut Bauen und Umwelt e.V.) (Independent verifier)
1 Environmental Product Declaration - Hansgrohe Group - Basin Faucets
2. Product
2.1 Product description/Product definition
Basin faucets
essentially comprise of a metal housing in most cases made of
• EN 15091:2014: Sanitary tapware – Electronic opening
brass, a plastic
and closing sanitary tapware
valve with ceramic discs and several assembly parts of various
• EN 60335-1:2012: Household and similar electrical
materials. The faucet
appliances - Safety - Part 1 Sanitary tapware –
surface is usually chrome-plated by means of various galvanic
Thermostatic mixing valves (PN
process stages.
10)
Some basin faucets are operated mechanically by handles and
• ISO 3822: Acoustics – Laboratory tests on noise
some electronically by
emission from appliances and equipment used in water
sensors.
supply installations
For the use
and application of the products the respective national
provisions at the place
of use apply, in Germany for example the building codes of the
Following
federal states
European directives and regulations may apply to electronic
and the corresponding national specifications.
operated taps,
depending on their functions:
The products comply with
the applicable standards and regulations listed below. 2.1.1
Mechanically operated basin faucets
Following
standards depending on the operating mechanism may apply to • 2011/65/EU (RoHS)
faucets and roughs • 2014/30/EU (EMC)
to prove product safety: • 2014/53/EU (RED)
• 2014/35/EU (LVD)
• 2009/125/EC (Ecodesign)
• 1275/2008/EC (Standby)
• EN 816:2017: Sanitary tapware – Automatic shut-off 2.2 Application
valves PN 10
2.2.1 Manual basin faucets are plumbing fixtures that mix hot
• EN 817:2008: Sanitary tapware – Mechanical mixing
and cold
valves (PN 10)
water, shut off water, and regulate the amount of water. They
• EN 200:2008: Sanitary tapware – Single taps and
are mechanically
combination taps for water supply systems of type 1 and
operated by handles and are used for hand washing in
type 2
bathrooms and toilets.
• ISO 3822: Acoustics – Laboratory tests on noise
2.2.2 Electronical basin faucets are plumbing fixtures that mix
emission from appliances and equipment used in water
hot and cold water, shut off
supply installations
water, and regulate the amount of water. They are automatically
operated by
sensors and are used for hand washing in bathrooms and
toilets.
2.3 Technical Data
The technical specifications of the products within the scope of
the EPD shall be listed, including the reference to the test
methods/test standards for each specification.
For products with CE marking, the technical specifications must
be specified in accordance with information in the declaration of
performance. The properties relevant to the product should be
specified in the table below. If no information is given for
properties, an explanation must be given in the background
2.1.2 report to the EPD as to why the property is not relevant to the
Electronically operated basin faucets product.
Constructional data
Following
standards apply to electronic operated taps to prove product
safety:
2 Environmental Product Declaration - Hansgrohe Group - Basin Faucets
Name Value Unit
Biocide
Maximum load temperature
65 °C products were added to this construction product or it has been
permanent operation
treated with
Maximum load temperature
90 °C biocide products (this then concerns a treated product as
temporary operation
defined by the (EU)
Flow rate (indications for Depending on the
m3/h Ordinance on Biocide Products No. 528/2012): no.
pressure range of 1-3 bar) product 0,09 to 1,2
Sound emissions < 30 dB 2.6 Manufacture
Performance
data of the product with respect to its characteristics in
accordance with the
relevant technical provision (no CE-marking).
2.4 Delivery status
The basin faucets
are delivered singularly packaged. The packaging is
customized to the size of
the product and supplies. Customers can order single products
or multiple
products with outer packaging. The products with the smallest
and the largest volume have dimensions between 155x85x285
mm and 227x247x460 mm.
2.5 Base materials/Ancillary materials
The material composition (incl. packaging) of an average basin
faucet is as follows:
Name Value Unit
Brass 48.9 % No. 1: The
Cardboard, Paper 18.2 % sand core for the base body is made.
Zinc 11.0 %
Polyphenylene 8.3 %
Other Plastics 7.9 %
No. 2: The
Stainless Steel 4.1 % body of the faucet is cast from brass using the sand core.
Other Materials 0.9 %
Steel 0.5 %
The parts which are made of brass contain between 0.2 and
No. 3:
1.4% lead.
After casting, the brass body is grinded and polished.
This product
contains substances listed in the candidate list (date:
17.12.2021) exceeding
No. 4: To protect
0.1 percentage by mass: Lead (CAS number 7439-92-1) as a
the product and make it durable, the body is galvanized with
component of the brass
chrome.
alloy has been on the candidate list of the Reach Regulation
(Regulation (EC)
No. 1907/2006) since 27.06.2018.
No. 5: Meanwhile,
the individual parts of the cartridge are assembled.
No. 6: The
product parts (chrome plated brass body, cartridge, chrome
This
plated handle and
product/article/at least one partial article contains other CMR
others) are assembled.
substances in
categories 1A or 1B which are not on the candidate list,
exceeding 0.1
percentage by mass: no.
No. 7: The
preassembled product is packed together with the remaining
components (like
fastening parts).
3 Environmental Product Declaration - Hansgrohe Group - Basin Faucets
wrench).
Any production
waste generated is disposed accordingly. In In the end
individual cases, the production may differ slightly from the the water temperature is adjusted by setting the cartridge (tools:
procedure (for standard
example, if the brass body is purchased and not manufactured hexagonal offset screwdriver).
in-house).
2.9 Packaging
2.7 Environment and health during manufacturing For product
Hansgrohe SE tries to keep the protection the basin faucets are individually packed in a
impact on people and the environment as low as possible when cardboard box, which
manufacturing its products. consists of approximately 80% recycled material. The
Hazards at workplaces are regularly cardboard is always
assessed and reduced to a minimum. printed with lead-free ink and in some cases additionally coated
with clear
topcoat. The inlay of the packaging consists of folded
cardboard, fiber form or
For example, in basic production, plastic bags, depending on the product.
sawing or grinding work is mainly carried out by robots, and in The
electroplating, packaging can be fully recycled.
chemicals are dosed automatically via appropriate pump
stations.
All
packaged products fit on a reusable euro pallet.
Emissions that are hazardous to
health are extracted directly at the source and cleaned by filter 2.10 Condition of use
systems. To protect
the basin faucets and make them durable, the body and handle
are made of
chrome-plated metal. Nevertheless, there are no unhealthy
Workplace and emission limits are contaminants in the
regularly monitored and are far below the prescribed limits. water and drinking water quality is guaranteed. To ensure the
longevity of the
product, it should be used daily and cleaned regularly.
2.11 Environment and health during use
To reduce environmental impact,
water and production waste are recycled wherever possible. Our
products do not emission any contaminants or substances that
are harmful to the
In addition, all production environment or health during the use phase.
sites are certified according to the DIN EN ISO standards
2.12 Reference service life
14001 (environment),
The quality and durability of our basin faucets is designed for a
50001 (energy), 45001 (occupational health and safety) and
product
9001 (quality).
life of about 20 years. Which on average is approximately the
Continuous improvement of environmental and occupational
duration of use
safety performance is
by the consumers. With few exceptions, all products have a
thus guaranteed.
five-year warranty. Furthermore, an after-sale service warranty
2.8 Product processing/Installation of 15 years is provided.
The basin faucets
2.13 Extraordinary effects
are installed to a basin with fastening bolts, centering rings and
Fire
shaft
The
fastenings (tool: standard screwdriver).
products are not classified as building materials (building
The flex
products) and are
hoses are connected (tool: standard wrench).
not subject to DIN 4102 and EN 13501-1.
Fire protection
Name Value
If it is
Building material class
included in the product, the drain is mounted on the basin and
Burning droplets
tested for leaks
(tool: standard screwdriver). Smoke gas development
Water
If a room in which the products
The jet offered by Hansgrohe are installed is flooded with water, the
regulator is inserted and tested with water (tool: standard electronic
4 Environmental Product Declaration - Hansgrohe Group - Basin Faucets
faucets may be destroyed. All other products are not affected in reverse order.
their All metal
function. components can be recycled (as scrap).
Mechanical destruction
If the surface of the coating is
destroyed by a mechanical stress, there is a possibility of All plastic
corrosion. components have a high calorific value and can be sent for
In the event of mechanical thermal recycling.
damage, the products may need to be replaced due to possible
sharp cut edges.
2.14 Re-use phase In
The basin faucets are not taken back by the manufacturer for countries where no thermal recycling or substance recycling is
the purpose of reuse. Users established,
can disassemble the products repeatedly within the reference disposal takes place via the waste incineration plant.
utilization period
and reuse it elsewhere. 2.16 Further information
Additional
2.15 Disposal information about our products can be found at
The waste code of the product is https://www.hansgrohe.com.
AVV 20 03 01. Disassembly
of the products consists of the same steps as assembly, in
3. LCA: Calculation rules
compared to the environmental impacts caused by the actual
3.1 Declared Unit production.
The results of
this EPD are valid for the following functional unit:
3.2 System boundary
This
Provide representative EPD follows the EPD type "cradle to gate - with
sanitary function for one (1) average basin faucet unit, allowing options". The following life cycle modules are declared:
the distribution of sanitary water with a
regulation of the flow rate and temperature, used in accordance Modules
with A1-A3:
the manufacturer's recommendations for a 20-year life,
following the manufacturer's operating instructions. An average
conditioned basin faucet is The
considered the baseline flow. product stage begins with considering the production of the
necessary raw
materials and energies, including all corresponding upstream
chains and the
actual procurement transports. Furthermore, the entire
manufacturing phase
was mapped, including the treatment of production waste until
the
Weighted end-of-waste status (EoW) was reached.
averaging based on production tonnages in 2021 is chosen as Green electricity from hydropower is used for the manufacturing
basis for creating processes in Germany. US electricity mix is used for the US
the environmental profile. 405 different basin faucets were production site. Chinese electricity mix is used for the Chinese
considered. production site, although electricity from photovoltaic is partly
used there.
Functional unit
Name Value Unit
Declared unit 1 pce. Module
Functional unit 1 pce. A4:
Functional unit with packaging 2.14 kg
Packaging 0.41 kg
All
Weight range of the products examined 0.86 - 4.5 kg
distribution transports to the customers were considered.
Other declared units are allowed if the conversion is shown
transparently.
Module
For IBU core EPDs (where clause 3.6 is part of the EPD): for A5:
average EPDs, an estimate of the robustness of the LCA
values must be made, e.g. concerning the variability of the
production process, geographical representativeness and the This
influence of background data and preliminary products module covers the installation process with the corresponding
5 Environmental Product Declaration - Hansgrohe Group - Basin Faucets
packaging waste and coating. For the incineration with
generated that needs to be disposed. energy recovery (thermal and electric) of waste, an r1 value
of > 0.6 is
Modules B1 & B3-B5: assumed. The net efficiency for the average waste incinerated
These modules were considered, but evaluated as not relevant is between 38 % and 44 %, depending on the type of waste
for the products and considered as zero. respectively the disposal data set.
Module B2: 3.4 Cut-off criteria
The effect
associated with the neglected mass shares is less than 5% of
Maintenance the effect
expenses are declared in this module and consist of weekly categories per module. The minimum limit of 1% total mass and
cleaning expenses, cartridge and battery replacement. the use of
renewable and nonrenewable primary energy is not exceeded.
Module
3.5 Background data
B6:
The LCA
This software GaBi 10.6 was used to model the life cycle. The entire
module considers the energy input required to bring water to a manufacturing
certain process, as well as energy consumption, were modelled on the
temperature for the use of a gas low temperature boiler basis of
(scenario B6/1) and for the use of an electric instantaneous manufacturer specific data.
water heater (scenario B6/2).
However, generic background datasets were used for the
upstream and downstream
Module processes. The majority of the background datasets used were
B7: taken from the
current version (2021.2) of the GaBi database. Ecoinvent
Version 3.6 (2019)
This datasets were only used when suitable GaBi datasets were not
module considers the water consumption that can be expected available.
depending on the
3.6 Data quality
function of the product family.
The background
datasets used for accounting purposes mainly originate from
the respective updated GaBi databases at the time of
Modules
calculation. The data for the examined products was captured
C1-C4:
on
The modules include the environmental impacts for dismantling
the basis of evaluations of internal production and
of the products and the treatment of the waste fractions until
environmental data, the collection of LCA relevant data within
the end-of-waste status (EoW) is reached, including the
the supply chain, as well as the evaluation of relevant data for
associated transports at the end of the product life cycle.
the energy supply. The collected
Module D:
data were checked for plausibility and consistency. Good
representativity can be assumed.
Identification
For the
of the benefits and costs of the product outside the system
assessment of the variability of the results, all products were
boundary. For waste,
balanced in
paper and plastics, these consist of energy credits from thermal
addition to the average product. See at chapter 6 for
utilization (A3,
explanation of the variability.
A5 and C3) in the form of the average European electricity mix
or thermal energy 3.7 Period under review
from natural gas. Recycling of paper, plastic and metal scrap
Life cycle assessment data were collected in
results in
2021.
credits of the respective raw materials for the primary material
portion of the input. The loads of the waste incineration and 3.8 Geographic Representativeness
recycling processes are assigned to the respective modules Land or region, in which the declared product system is
(A3, A5 and C3) and manufactured, used or handled at the end of the product´s
not to module D. lifespan: Global
3.3 Estimates and assumptions
Energy and water consumption, material amount 3.9 Allocation
for coating as well as waste during production could only be For the production process nearly all raw materials, precursors
determined on and supplies could be assigned to the declared product.
concrete, existing products and not on the average product. Energy, water, galvanization process and production waste
The highest value of all inputs and outputs for were assigned to the highest value of either the heaviest,
energy, waste and coating of the top seller, the lightest and the lightest or most sold product of the product group. No
heaviest byproducts are produced and no allocation is required.
product was used for the calculation of energy, water, waste Some of the brass losses from brass processing in module A3
6 Environmental Product Declaration - Hansgrohe Group - Basin Faucets
are directly reused by Hansgrohe and are modelled as a closed Deconstructed product at the end of life:
loop. Another part of the brass losses (brass particles and Since the product is predominantly made of
dusts) is disposed of as waste (without debits and credits). metal, it is assumed that most of its metallic components are
Credits for plastics, paper and cardboard recycled in A5 and recycled. 95 % of the non-metallic components are incinerated
metallurgical waste in C3 are credited in module D. with energy recovery and 5 % are disposed in landfill. For the
Credits for the energy recovery of incinerated production waste metal components, it is assumed that 90 % are sent for material
in A1-3, paper, cardboard and plastics in A5 and plastics and recycling, 5 % for incineration with energy recovery (C3) and 5
other materials in C3 are credited in module D. % are disposed in landfill (C4).
The loads for waste water treatment and waste disposal of core
sand, waste oil and hazardous waste from the manufacturing 3.10 Comparability
phase are allocated to module A3. Basically, a comparison or an evaluation of EPD data is only
possible if all the data sets to be compared were created
Packaging: according to EN 15804 and the building context, respectively
For paper and cardboard, recycling (91 %) and energy recovery the product-specific characteristics of performance, are taken
(9 %) are considered on a pro rata basis. For plastic, a into account.
proportionate recycling (52 %), energy recovery (48 %) The used background database has to be mentioned.
considered, based on Eurostat.
4. LCA: Scenarios and additional technical information
Characteristic product properties of biogenic carbon The cartridge is
The biogenic carbon content quantifies the amount of biogenic replaced once during its service life. And the battery of the
carbon in a construction product leaving the factory gate, and it electronic basin faucets must be replaced every two years
shall be separately declared for the product and for any (electronic basin faucets
accompanying packaging. comprise 0.5% of the total basin faucets).
If the total mass of biogenic carbon containing materials is less
Name Value Unit
than 5 % of the total mass of the product and accompanying
Maintenance cycle (cleaning) 1040 Number/RSL
packaging, the declaration of biogenic carbon content may be
omitted. The mass of packaging containing biogenic carbon Water consumption/Cycle weekly 0.5 Liter/cycle
shall always be declared. (cleaning)
Soap concentration (cleaning) 1.5 %
Information on describing the biogenic Carbon Content at Water consumption (cleaning) 0.52 m3
factory gate Auxiliary Soap/Tensides (cleaning) 7.8 kg
The biogenic carbon content was calculated based on the Maintenance Cycle (battery replacement) 10 Number/RSL
factors from the
Battery Lithium 6V (battery replacement) 0.0021 kg/RSL
Thünen Intitute.
Maintenance Cycle (cartridge
Name ValueUnit 1 Number/RSL
replacement)
Biogenic carbon content in accompanying kg
0.15 Cartridge (cartridge replacement) 0.0581 kg/RSL
packaging C
Note: 1 kg of biogenic carbon is equivalent to 44/12 kg of CO .
2 In case a reference service life according to applicable ISO
standards is declared then the assumptions and in-use
conditions underlying the determined RSL shall be declared. In
The following technical information is a basis for the declared addition, it shall be stated that the RSL applies to the reference
modules. conditions only.
Transport to the building site (A4)
The same holds for a service life declared by the manufacturer.
Name ValueUnit
Corresponding information related to in-use conditions needs
Transport distance (Truck) 439 km
not be provided if a service life taken from the list of service life
Capacity utilisation (including empty runs) (Truck) 55 % by BNB is declared.
Transport distance (Container Ship) 6871 km
Capacity utilisation (Container Ship) 80 % Service life
Hansgrohe
Installation into the building (A5)
SE declares a Service Life of 20 years as an empirical value for
Except of fitting grease, no the basin faucets when used in accordance with the care
additional resources or energy are required for the installation. instructions. This value is
The packaging is disposed based on their technical service centre's statistics on service
either by recycling or incineration. life in the
Name Value Unit market and complaints.
Packaging (Paper, cardboard and plastic) 0.407 kg
Grease 0.01 kg Name Value Unit
Life Span according to the manufacturer 20 a
Maintenance (B2)
For Operational energy use (B6) and Operational water use
module B2, it is assumed that a weekly cleaning of the product (B7)
takes place,
with 0.5 liter of water containing 1.5% soap.
7 Environmental Product Declaration - Hansgrohe Group - Basin Faucets
Name Value Unit
Water consumption 53.4 m3 Reuse, recovery and/or recycling potentials (D), relevant
scenario information
Energy demand 2486 kWh
The energy generated from energy recovery as well as recycled
materials are assigned to module D as possible potentials or
End of life (C1-C4)
avoided loads in subsequent systems. Credits are only given
Name Value Unit for the primary portion of the inputs.
Collected separately waste type 1.722 kg
Recycling 1.236 kg
Energy recovery 0.4 kg
Landfilling 0.087 kg
8 Environmental Product Declaration - Hansgrohe Group - Basin Faucets
5. LCA: Results
The following
table shows the result of the LCA for 1 piece of an average basin faucet. The
results in the B-module are based on a lifetime of 20 years. Scenario B6/1 shows the result for the use of a gas low temperature boiler.
Scenario B6/2 shows the result for the use of an electric instantaneous water heater.
DESCRIPTION OF THE SYSTEM BOUNDARY (X = INCLUDED IN LCA; MND = MODULE OR INDICATOR NOT DECLARED; MNR
= MODULE NOT RELEVANT)
Benefits and
Construction loads beyond
Product stage Use stage End of life stage
process stage the system
boundaries
la ire ta m w a Ry lp p u s tro p s n a rT g n iru tc a fu n a M e h t m o rf tro p s n a rTe tis e h t o t e ta g y lb m e s s A e s U e c n a n e tn ia M ria p e R tn e m e c a lp e R tn e m h s ib ru fe R y g re n e la n o ita re p Oe s u re ta w la n o ita re p Oe s u n o itc u rts n o c -e Dn o itilo m e d tro p s n a rT g n is s e c o rp e ts a W la s o p s iD -e s u e R-y re v o c e R-g n ilc y c e Rla itn e to p
A1 A2 A3 A4 A5 B1 B2 B3 B4 B5 B6 B7 C1 C2 C3 C4 D
X X X X X X X X X X X X X X X X X
RESULTS OF THE LCA - ENVIRONMENTAL IMPACT according to EN 15804+A2: 1 piece average basin faucet incl. packaging
Parameter Unit A1-A3 A4 A5 B1 B2 B3 B4 B5 B6/1 B6/2 B7 C1 C2 C3 C4 D
GWP-total kg CO 2 5.75E 2.04E- 6.38E- 0 2.59E 0 0 0 6.64E 9.89E 3.16E 0 2.93E- 8.53E- 4.6E-03 -3.52E
eq +00 01 01 +01 +02 +02 +01 02 01 +00
GWP-fossil kg CO 2 6.3E+00 2.03E- 6.98E- 0 1.99E 0 0 0 6.64E 9.88E 3.16E 0 2.91E- 8.53E- 4.6E-03 -2.95E
eq 01 02 +01 +02 +02 +01 02 01 +00
GWP- kg CO 2 -5.68E- 0 5.68E- 0 0 0 0 0 0 0 0 0 0 0 0 -5.58E-
biogenic eq 01 01 01
GWP-luluc kg CO 2 1.43E-02 6.55E- 8.14E- 0 6.02E 0 0 0 3.36E- 1.4E+00 2.56E- 0 2.39E- 9.26E- 4.38E- -8.85E-
eq 04 05 +00 02 02 04 05 06 03
kg CFC11 2.84E- 3.27E- 1.09E- 2.39E- 2.99E- 5.77E- 1.08E- -1.15E-
ODP 1.03E-08 0 0 0 0 2.37E-11 0 8.31E-11
eq 17 16 06 13 13 18 17 08
4.66E- 8.05E- 6.72E- 4.07E- 2.06E 7.78E- 4.88E- 1.86E- 1.44E- -3.55E-
AP mol H+ eq 6.1E-02 0 0 0 0 0
03 05 02 01 +00 02 05 04 05 02
EP- 2.65E- 6.12E- 6.06E- 2.65E- 3.37E- 8.68E- 1.46E- -1.13E-
kg P eq 3.78E-05 1.3E-07 0 0 0 0 0 2.3E-07
freshwater 07 04 05 03 02 08 07 05
1.25E- 2.07E- 1.53E- 1.73E- 4.88E- 1.48E- 1.92E- 5.98E- 3.64E- -3.75E-
EP-marine kg N eq 7.85E-03 0 0 0 0 0
03 05 02 01 01 01 05 05 06 03
1.37E- 2.44E- 1.83E- 1.89E 5.13E 2.33E- 8.18E- 3.86E- -3.98E-
EP-terrestrial mol N eq 8.34E-02 0 0 0 0 0 2.2E-04
02 04 01 +00 +00 01 04 05 02
kg
3.47E- 6.09E- 5.05E- 1.33E 5.96E- 4.36E- 1.61E- 1.14E- -1.14E-
POCP NMVOC 2.32E-02 6.5E-05 0 0 0 0 0
03 02 01 +00 02 05 04 05 02
eq
1.08E- 5.87E- 2.36E- 3.57E- 2.91E- 4.13E- 2.59E- 1.41E- 3.14E- -2.12E-
ADPE kg Sb eq 2.86E-03 0 0 0 0 0
08 09 05 05 04 06 09 08 10 03
9.44E 2.56E 7.88E- 4.56E 1.14E 1.76E 3.26E 3.89E- 6.23E- 6.61E- -3.45E
ADPF MJ 0 0 0 0 0
+01 +00 01 +02 +04 +04 +02 01 01 02 +01
m3 world
9.09E 9.29E- 1.07E- 6.96E 1.74E 1.59E 9.74E 2.71E- 8.52E- -6.45E
WDP eq 0 0 0 0 0 -5E-05
+00 04 02 +00 +00 +02 +00 04 02 +00
deprived
GWP = Global warming potential; ODP = Depletion potential of the stratospheric ozone layer; AP = Acidification potential of land and water; EP =
Eutrophication potential; POCP = Formation potential of tropospheric ozone photochemical oxidants; ADPE = Abiotic depletion potential for non-fossil
resources; ADPF = Abiotic depletion potential for fossil resources; WDP = Water (user) deprivation potential)
RESULTS OF THE LCA - INDICATORS TO DESCRIBE RESOURCE USE according to EN 15804+A2: 1 piece average basin
faucet incl. packaging
Parameter Unit A1-A3 A4 A5 B1 B2 B3 B4 B5 B6/1 B6/2 B7 C1 C2 C3 C4 D
1.74E 6.57E 9.91E 9.59E -1.09E
PERE MJ 6.63E-02 0 9.4E+01 0 0 0 8.1E+03 0 2.24E-022.82E-01 4.8E-03
+01 +00 +01 +01 +01
6.47E -6.47E
PERM MJ 0 0 0 0 0 0 0 0 0 0 0 0 0 0
+00 +00
2.39E 9.91E 9.59E -1.09E
PERT MJ 6.63E-029.38E-02 0 9.4E+01 0 0 0 8.1E+03 0 2.24E-022.82E-01 4.8E-03
+01 +01 +01 +01
8.11E 2.56E 4.56E 1.14E 1.76E 3.26E 1.23E -3.46E
PENRE MJ 1.9E+00 0 0 0 0 0 3.91E-01 6.82E-01
+01 +00 +02 +04 +04 +02 +01 +01
1.34E -1.11E -1.17E -6.15E-
PENRM MJ 0 0 0 0 0 0 0 0 0 0 0 0
+01 +00 +01 01
9.45E 2.56E 4.56E 1.14E 1.76E 3.26E -3.46E
PENRT MJ 7.89E-01 0 0 0 0 0 3.91E-016.23E-01 6.62E-02
+01 +00 +02 +04 +04 +02 +01
SM kg 8.15E-01 0 0 0 2.46E-03 0 0 0 0 0 0 0 0 0 0 9.4E-01
-4.73E-
RSF MJ 5.64E-25 0 0 0 0 0 0 0 0 0 0 0 0 0 0
25
9 Environmental Product Declaration - Hansgrohe Group - Basin Faucets
NRSF MJ 0 0 0 0 0 0 0 0 0 0 0 0 0 0 0 0
7.89E -1.45E-
FW m3 2.12E-017.84E-052.94E-04 0 1.63E-01 0 0 0 1.11E-01 2.78E-01 0 2.56E-052.11E-03 7.74E-07
+00 01
PERE = Use of renewable primary energy excluding renewable primary energy resources used as raw materials; PERM = Use of renewable primary
energy resources used as raw materials; PERT = Total use of renewable primary energy resources; PENRE = Use of non-renewable primary energy
excluding non-renewable primary energy resources used as raw materials; PENRM = Use of non-renewable primary energy resources used as raw
materials; PENRT = Total use of non-renewable primary energy resources; SM = Use of secondary material; RSF = Use of renewable secondary fuels;
NRSF = Use of non-renewable secondary fuels; FW = Use of net fresh water
RESULTS OF THE LCA – WASTE CATEGORIES AND OUTPUT FLOWS according to EN 15804+A2:
1 piece average basin faucet incl. packaging
Parameter Unit A1-A3 A4 A5 B1 B2 B3 B4 B5 B6/1 B6/2 B7 C1 C2 C3 C4 D
-1.26E-
HWD kg 1.88E-066.78E-116.77E-11 0 8.5E-03 0 0 0 2.13E-064.65E-06 6.7E-08 0 2.06E-111.73E-101.17E-11
05
1.12E 1.25E
NHWD kg 3.17E-043.28E-03 0 6.97E-01 0 0 0 1.5E+00 5.2E+01 0 6.13E-05 5.2E-02 8.6E-02 -7.2E-01
+00 +01
2.62E -1.63E-
RWD kg 2.93E-03 3.6E-06 1.75E-05 0 4.21E-03 0 0 0 2.52E-02 2.67E-02 0 7.08E-073.97E-057.58E-07
+00 03
CRU kg 0 0 0 0 0 0 0 0 0 0 0 0 0 0 0 0
1.24E
MFR kg 0 0 3.65E-01 0 1.83E-03 0 0 0 0 0 0 0 0 0 0
+00
MER kg 0 0 0 0 9.01E-04 0 0 0 0 0 0 0 0 0 0 0
EEE MJ 1.28E-01 0 1.57E-01 0 1.58E-01 0 0 0 0 0 0 0 0 2.56E-022.57E-04 0
EET MJ 3.94E-01 0 2.82E-01 0 2.87E-01 0 0 0 0 0 0 0 0 4.8E-02 0 0
HWD = Hazardous waste disposed; NHWD = Non-hazardous waste disposed; RWD = Radioactive waste disposed; CRU = Components for re-use;
MFR = Materials for recycling; MER = Materials for energy recovery; EEE = Exported electrical energy; EET = Exported thermal energy
RESULTS OF THE LCA – additional impact categories according to EN 15804+A2-optional:
1 piece average basin faucet incl. packaging
Parameter Unit A1-A3 A4 A5 B1 B2 B3 B4 B5 B6/1 B6/2 B7 C1 C2 C3 C4 D
Disease 6.02E- 7.83E- 5.17E- 3.32E- 2.83E- 1.73E- 8.75E- 3.05E- 1.65E- 1.53E- -3.36E-
PM 0 0 0 0 0
incidence 07 08 10 06 06 05 07 10 09 10 07
kBq U235 2.36E- 2.15E 4.21E 1.04E- 4.03E- 1.09E- -1.09E
IR 1.4E+00 5.2E-04 0 0 0 0 4E+00 4.3E+02 0
eq 03 +00 +00 04 03 04 +00
9.52E 1.87E 4.96E- 2.05E 1.56E 7.39E 2.89E- 4.03E- -2.91E
ETP-fw CTUe 0 0 0 0 4.6E+03 0 3.11E-02
+01 +00 01 +02 +02 +03 01 01 +01
2.72E- 3.33E- 2.09E- 1.56E- 5.84E- 2.42E- -7.01E-
HTP-c CTUh 1.3E-07 3.61E-111.12E-11 0 0 0 0 0 1.54E-11
08 08 07 07 12 12 09
3.95E- 1.79E- 4.96E- 7.59E- 3.52E- 1.61E- 1.15E- 2.31E- -2.31E-
HTP-nc CTUh 0 0 0 0 7.9E-06 0 3.11E-10
07 09 10 07 06 05 09 10 07
4.69E 3.69E- 1.01E- 3.18E 6.63E 5.55E 1.61E 1.34E- -2.85E
SQP SQP 0 0 0 0 0 2.4E-01 4.8E-03
+01 01 01 +02 +01 +03 +02 01 +01
PM = Potential incidence of disease due to PM emissions; IR = Potential Human exposure efficiency relative to U235; ETP-fw = Potential comparative
Toxic Unit for ecosystems; HTP-c = Potential comparative Toxic Unit for humans (cancerogenic); HTP-nc = Potential comparative Toxic Unit for humans
(not cancerogenic); SQP = Potential soil quality index
Disclaimer 1 – for the indicator “Potential Human exposure efficiency relative to U235”. This impact category deals mainly with the
eventual impact of low-dose ionizing radiation on human health of the nuclear fuel cycle. It does not consider effects due to possible
nuclear accidents, occupational exposure or radioactive waste disposal in underground facilities. Potential ionizing radiation from the
soil, radon and from some construction materials is also not measured by this indicator.
Disclaimer 2 – for the indicators “abiotic depletion potential for non-fossil resources”, “abiotic depletion potential for fossil resources”,
“water (user) deprivation potential, deprivation-weighted water consumption”, “potential comparative toxic unit for ecosystems”,
“potential comparative toxic unit for humans – cancerogenic”, “Potential comparative toxic unit for humans - not cancerogenic”,
“potential soil quality index”. The results of this environmental impact indicator shall be used with care as the uncertainties on these
results are high as there is limited experience with the indicator.
6. LCA: Interpretation
10 Environmental Product Declaration - Hansgrohe Group - Basin Faucets
The dominance analysis shows that
modules B2, B6 and B7 are the dominant life cycle stages in 3,050,479 basin faucets of 405
most of the different product types were produced. For the assessment of
categories. The contribution of B2 is due to the demand of soap the variability of
and water for the results, all products were balanced and compared to the
cleaning. Module B6 dominates most of the indicators due to average product
the energy demand weighted by production volume.
for water heating and module B7 has a high contribution to
EPfreshwater
due to the wastewater treatment. The module A1-A3 has a very
low contribution The different types of products all
to all categories except of ADPE. In this indicator the provision have the same function and differ mainly in terms of design,
of brass has which has an
the largest contribution. influence on construction and materials used. The basic
structure of the
product types is always similar. Material type and quantity
proportions do not
The end-of-life stage has no differ much, as also shown in the average material composition
significant influence on the environmental indicators. table.
The environmental burdens from the The deviation of the GWP fossil in
transports (modules A4 and C2) account for less than 1% of the modules A1-C4 has a maximum of 90% and a minimum of -
total burdens of 60% with scenario B6/1
the respective indicators in all cases. (gas low temperature boiler). The variation of the GWP fossil in
modules A1-C4
has a maximum of 91% and a minimum of -61% with scenario
B6/2 (electric
The possible potentials of avoided instantaneous water heater).
loads of subsequent systems (module D) lie outside the
considered system
boundaries and relate exclusively to credits from recycling and
thermal For an average scenario, where 50%
recycling by means of incineration with energy recovery of the of water is heated with gas low temperature boiler and 50%
different with electric
materials. instantaneous water heater, 2% of the basin faucets produced
are above the
11 Environmental Product Declaration - Hansgrohe Group - Basin Faucets
average GWP fossil value. Whereas 98% reflect the average or the average is mainly caused by the flow rate in module B7.
are lower than the The higher the
average. deviation from the average GWP, the higher the flow rate. The
flow rate ranges
between 1.9 and 9.7 l/min. Consequently, the production phase
Modules has a minor
B6 and B7 account for more than 90% of the GWP indicator. influence on the LCA results.
The deviation from
7. Requisite evidence
The drinking
• KTW: Assessment basis for plastics and other organic
water regulation determines the quality of drinking water at the
materials in contact with drinking water
point of
• Elastomer guideline: Guideline for the hygienic
withdrawal. This result in requirements for used materials in
assessment of elastomers in contact with drinking water
drinking water
• Thermoplastic elastomers: Recommendation for the
installations in general and therefore in sanitary fittings in
hygienic assessment of products made of thermoplastic
particular.
elastomers in contact
with drinking water (TPE transition recommendation)
• Ceramics: draft assessment basis for enamels and
ceramic materials: assessment basis for enamels and
All materials
ceramic materials in
used by Hansgrohe SE, which are in contact with drinking
contact with drinking water (enamel/ceramic
water, fulfill the
assessment basis)
drinking water regulation.
• Lubricants: Guideline for the hygienic assessment of
lubricants in contact with drinking water (sanitary
lubricants), (Lubricant
Guideline)
Regulations for
metals (Europe-wide):
• Acceptance of metallic materials used for products in
contact with drinking water: 4MS Common Approach Regulation for
other materials (France):
• ACS: Attestation de Conformité Sanitaire (plastics,
elastomers, metals)
- Part A – Procedure for the acceptance
Regulation for
- Part B – 4MS Common Composition List
other materials (UK):
• BS 69 20: Suitability of non-metallic products for use
in contact with water intended for human consumption
• Metal recommendation
with regard to their
of the federal environment agency: metal materials
effect on the quality of water (plastics, elastomers)
suitable for drinking water
hygiene
Products of the
Hansgrohe SE are therefore uncritical to use with any drinking
Regulations for
water.
other materials (Germany):
8. References
Standards
ISO 3822
EN 200 ISO 3822: Acoustics – Laboratory tests on noise emission from
EN 200:2008: Sanitary tapware – Single taps and combination appliances and equipment used in water supply installations
taps for water supply systems of type 1 and type 2
EN 816 DIN 4102-1
EN 816:2017: Sanitary tapware – Automatic shut-off valves PN DIN 4102-1: Fire behaviour of building materials and building
10 components - Part 1: Building materials; concepts,
requirements and tests. 1998-05
EN 817
EN 817:2008: Sanitary tapware – Mechanical mixing valves DIN EN ISO 9001
(PN 10) DIN EN ISO 9001:2015: Quality management systems -
12 Environmental Product Declaration - Hansgrohe Group - Basin Faucets
Requirements (ISO 9001:2015) Ecoinvent
ecoinvent 3.6 Database on Life Cycle Inventories (Life Cycle
Inventory data), ecoinvent Association, Zürich, 2020
DIN EN 13501-1
DIN EN 13501-1:2019-05: Fire classification of construction
products and building elements - Part 1: Classification using EU Ordinance on biocide Products No. 528/2012
data from reaction to fire tests; German version EN 13501- European Parliament, 2012. Regulation (EU) no 528/2012 of
1:2018 the European parliament and of the council of 22 May 2012
concerning the making available on the market and use of
biocidal products
DIN EN ISO 14001
DIN EN ISO 14001:2015, Environmental management systems
— Requirements with guidance for use, 2015-09
DIN EN ISO 14025 Eurostat
DIN EN ISO 14025: Environmental labels and declarations -
Type III environmental declarations - Principles and procedures,
2011-10
Eurostat, last update 26/10/2021 on
https://ec.europa.eu/eurostat/databrowser/view/ten00063/default/table?
EN 15091 ang=en
EN 15091:2014: Sanitary tapware – Electronic opening and
closing sanitary tapware
EN 15804
DIN EN 15804:2012+A2:2019+AC:2021: Sustainability of GaBi
construction works - Environmental product declarations - Core GaBi 10.6, GaBi Software System and Database for Life Cycle
rules for the product category of construction products Engineering version 2021.2, Sphera Solutions GmbH,
Leinfelden-Echterdingen, 1992-2021
DIN EN ISO 45001
DIN EN ISO 45001:2018: Occupational health and safety IBU 2021
management systems — Requirements with guidance for use. General Instructions for the EPD programme of Institut Bauen
2018-03 und Umwelt e.V. Version 2.0, Berlin: Institut Bauen und Umwelt
e.V., 2021, www.ibu-epd.com
DIN EN ISO 50001
DIN EN ISO 50001:2018: Energy management systems — PCR Part A
Requirements with guidance for use. 2018-08 Institut Bauen und Umwelt e.V. (IBU), Product Category Rules
for Building-Related Products and Services. Part A: Calculation
rules for the life cycle assessment and requirements on the
EN 60335 project report. Version 2.1, Berlin, 11/2021
EN 60335-1:2012: Household and similar electrical appliances -
Safety - Part 1 Sanitary tapware – Thermostatic mixing valves
(PN 10) PCR Part B
Institut Bauen und Umwelt e.V. (IBU), Requirements on the
EPD for fittings and showers. Version 1.1, Berlin, 03/2022
Further References
Thünen Institute
AVV
Draft General administrative provision relating to the Order on
the European list of wastes (Waste List Order – German Diestel, Sylvia / Weimar, Holger: Der Kohlenstoffgehalt in
designation: AVV) of 10 December 2001. Holz- und Papierprodukten - Herleitung und
Umrechnungsfaktoren. Thünen Working Paper 38. Johann
Heinrich von Thünen-Institut. Hamburg, 2014
ECHA The literature referred to in the Environmental Product
European Chemicals Agency (ECHA) Candidate List of Declaration must be listed in full.Standards already fully quoted
Substances of Very High Concern (SVHC) for Authorisation in the EPD do not need to be listed here again.
https://echa.europa.eu/de/candidate-listtable The current version of PCR Part A and PCR Part B of the PCR
document on which they are based must be referenced.
13 Environmental Product Declaration - Hansgrohe Group - Basin Faucets
Publisher
Institut Bauen und Umwelt e.V. +49 (0)30 3087748- 0
Hegelplatz 1 info@ibu-epd.com
10117 Berlin www.ibu-epd.com
Germany
Programme holder
Institut Bauen und Umwelt e.V. +49 (0)30 3087748- 0
Hegelplatz 1 info@ibu-epd.com
10117 Berlin www.ibu-epd.com
Germany
Author of the Life Cycle Assessment
brands & values GmbH +49 421 70 90 84 33
Altenwall 14 info@brandsandvalues.com
28195 Bremen www.brandsandvalues.com
Germany
Owner of the Declaration
Hansgrohe Group +49 7836 51-0
Auestr. 5-9 info@hansgrohe-group.com
77761 Schiltach www.hansgrohe-group.com
Germany
14 Environmental Product Declaration - Hansgrohe Group - Basin Faucets
