ENVIRONMENTAL PRODUCT DECLARATION
as per ISO 14025 and EN 15804+A2
Owner of the Declaration dormakaba International Holding GmbH
Publisher Institut Bauen und Umwelt e.V. (IBU)
Programme holder Institut Bauen und Umwelt e.V. (IBU)
Declaration number EPD-DOR-20210152-CBA2-EN
Issue date 16.07.2021
Valid to 15.07.2026
BEST HD8000
dormakaba
www.ibu-epd.com | https://epd-online.com
General Information
dormakaba BEST HD8000
Programme holder Owner of the declaration
IBU – Institut Bauen und Umwelt e.V. dormakaba International Holding GmbH
Hegelplatz 1 DORMA Platz 1
10117 Berlin 58256 Ennepetal
Germany Germany
Declaration number Declared product / declared unit
EPD-DOR-20210152-CBA2-EN 1 door closer (1 piece) of the BEST HD8000 series
This declaration is based on the product category rules: Scope:
Building Hardware products, 01.08.2021 This Environment Product Declaration refers to a specific door closer
(PCR checked and approved by the SVR) manufactured by dormakaba Production GmbH & Co. KG. The production
site is located in Singapore. The LCA results are valid for the variants
HD8016 and HD8056.
Issue date
The data represents the year 2019.
16.07.2021
The owner of the declaration shall be liable for the underlying information
and evidence; the IBU shall not be liable with respect to manufacturer
information, life cycle assessment data and evidences.
Valid to
15.07.2026 The EPD was created according to the specifications of EN 15804+A2. In
the following, the standard will be simplified as EN 15804.
Verification
The standard EN 15804 serves as the core PCR
Independent verification of the declaration and data according to ISO
14025:2011
internally X externally
Dipl.-Ing. Hans Peters
(Chairman of Institut Bauen und Umwelt e.V.)
Florian Pronold Dr.-Ing. Wolfram Trinius,
(Managing Director Institut Bauen und Umwelt e.V.) (Independent verifier)
1 Environmental Product Declaration - dormakaba - BEST HD8000
Product
Performance data of the product with respect to its
Product description/Product definition characteristics in accordance with the relevant technical
The HD8000 series are non-handed surface applied door provision which can be applied are mentioned above.
closers with adjustable spring power (size 1-6 and size 5-6) and
backcheck that controls opening motion during abusive or The plant in Singapore is certified to the Quality Management
abrupt opening. Supported by a full complement of optional system ISO 9001, which ensures consistent quality of
arms, plates, and brackets, the door closers provide the dormakaba's products.
flexibility needed to meet the demands of commercial and
institutional applications, including Americans with Disabilities The Environmental Management System in the Singapore
Act (ADA) barrierfree accessibility requirements (only size 1-6). production is certified to ISO 14001 and the Energy
The door closers are available with plastic and metal cover. For Management System to ISO 50001.
the use and application of the product the respective national
provisions at the place of use apply. The HD8000 is a Base materials/Ancillary materials
Underwriters Laboratories (UL) listed product. Name Value Unit
Steel 62 %
The standards which can be applied are the following:
Aluminum 25 %
• ANSI/BHMA 156.4:2019
Plastic 4 %
• ANSI/ICC A117.1:2017
Oil 4 %
• UL 10C:2016
• ADA (version 1-6) Others (Lacquer) 4 %
The product/s include/s partial articles which contain
Application
substances listed in the Candidate List of REACH Regulation
The HD8000 series closers are designed for commercial and
1907/2006/EC (date: 19.01.2021) exceeding 0.1 percentage by
institutional applications, including ADA barrier-free accessibility
mass: yes
requirements. They are suitable for use on hollow metal,
aluminum
• Lead (Pb): 7439-92-1 (CAS-No.) is included in some of
and wood doors and can be used for fire doors.
the alloys used. The concentration of lead in each
Technical Data individual alloy does not exceed 4.0% (by mass).
The door closers have following technical properties:
The Candidate List can be found on the ECHA website
address: https://echa.europa.eu/de/home.
Reference service life
The reference service life of the HD8000 Series door closers
depends on the traffic pattern and degree of usage of the door.
These closers are rated to ANSI Grade 1, meaning they are
designed to withstand a minimum of 1,500,000 cycles. The
reference service life amounts for 20 years.
LCA: Calculation rules
The difference in product weight for the two-door
Declared Unit closer types is approx. 4%. The product with the highest weight
The declared unit is 1 piece of the product: BEST HD 8000 is
series. declared in this EPD representing the entire product series.
System boundary
Declared unit and mass reference
The type of EPD is: cradle to gate with options, modules C1–
Name Value Unit
C4, and module D (A1–A3 + C + D and additional modules: A4
Declared unit 1 piece/product + A5)
Conversion factor to 1 kg kg per declared
4.12 -
product Production - Module A1-A3
Mass of declared Product 4.12 kg The product stage includes:
2 Environmental Product Declaration - dormakaba - BEST HD8000
— A1, raw material extraction, processing and mechanical provision and all transport, provision of all materials, products
treatments, processing of secondary material input (e.g. and related energy and water use.
recycling processes), — A2, transport to the manufacturer, — Module D (Benefits and loads beyond the system boundary)
A3, manufacturing and assembly including provision of all includes:
materials, products and energy, as well as waste processing up — D, recycling potentials, expressed as net impacts and
to the end-of waste state. benefits.
Construction stage - Modules A4-A5
The construction process stage includes: Geographic Representativeness
— A4, transport to the building site; — A5, installation into the Land or region, in which the declared product system is
building; including provision of all materials, products and manufactured, used or handled at the end of the product´s
energy, as well as waste processing up to the end-of waste lifespan: Singapore
state or disposal of final residues during the construction
process stage.
Comparability
Basically, a comparison or an evaluation of EPD data is only
End-of-life stage– Modules C1-C4 and D
possible if all the data sets to be compared were created
The end-of-life stage includes:
according to EN 15804 and the building context, respectively
— C1, de-construction, demolition:
the product-specific characteristics of performance, are taken
— C2, transport to waste processing; — C3, waste processing
into account.
for reuse, recovery and/or recycling; — C4, disposal; including
LCA: Scenarios and additional technical information
Installation into the building (A5)
Characteristic product properties of biogenic carbon
Name ValueUnit
Information on describing the biogenic Carbon Content at
Output substances following waste treatment on
factory gate 0.25 kg
site (packaging)
Name ValueUnit
kg End of life (C1-C4)
Biogenic carbon content in product 0.01
C C1: The product dismantling from the building is done manually
Biogenic carbon content in accompanying kg without environmental burden.
0.09
packaging C C2: Transport to waste treatment at end of life is 50km.
Note: 1 kg of biogenic carbon is equivalent to 44/12 kg of CO . Name Value Unit
2
Recycling 4.12 kg
Reuse, recovery and/or recycling potentials (D), relevant
Additional technical information for the declared modules.
scenario information
Transport to the building site (A4)
Name Value Unit
Name Value Unit
Recycling 100 %
Litres of fuel truck (per piece) 0.008l/100km
Collection rate is 100%.
Transport distance truck 100 km
Capacity utilisation (including empty runs)
55 %
average
3 Environmental Product Declaration - dormakaba - BEST HD8000
LCA: Results
DESCRIPTION OF THE SYSTEM BOUNDARY (X = INCLUDED IN LCA; MND = MODULE OR INDICATOR NOT DECLARED; MNR
= MODULE NOT RELEVANT)
Benefits and
Construction loads beyond
Product stage Use stage End of life stage
process stage the system
boundaries
la ire ta m w a Ry lp p u s tro p s n a rT g n iru tc a fu n a M e h t m o rf tro p s n a rTe tis e h t o t e ta g y lb m e s s A e s U e c n a n e tn ia M ria p e R tn e m e c a lp e R tn e m h s ib ru fe R y g re n e la n o ita re p Oe s u re ta w la n o ita re p Oe s u n o itc u rts n o c -e Dn o itilo m e d tro p s n a rT g n is s e c o rp e ts a W la s o p s iD -e s u e R-y re v o c e R-g n ilc y c e Rla itn e to p
A1 A2 A3 A4 A5 B1 B2 B3 B4 B5 B6 B7 C1 C2 C3 C4 D
X X X X X MND MND MNR MNR MNR MND MND X X X X X
RESULTS OF THE LCA - ENVIRONMENTAL IMPACT according to EN 15804+A2: 1 door closer
Parameter Unit A1-A3 A4 A5 C1 C2 C3 C4 D
GWP-total kg CO 2 eq 1.06E+01 3.67E-02 3.16E-01 0 1.74E-02 5.69E-01 4.93E-03 -4.63E+00
GWP-fossil kg CO 2 eq 1.1E+01 3.51E-02 1.29E-02 0 1.66E-02 5.69E-01 4.9E-03 -4.62E+00
GWP-biogenic kg CO 2 eq -3.83E-01 1.62E-03 3.03E-01 0 7.68E-04 1.33E-05 1.67E-05 -5.4E-03
GWP-luluc kg CO 2 eq 9.93E-03 8.35E-07 5.4E-06 0 3.96E-07 3.22E-05 1.41E-05 -5.52E-04
ODP kg CFC11 eq 5.76E-10 3.7E-18 5.86E-17 0 1.75E-18 2.87E-16 1.82E-17 -1.54E-11
AP mol H+ eq 4.13E-02 3.51E-05 8.8E-05 0 1.66E-05 1.01E-04 3.51E-05 -1.43E-02
EP-freshwater kg P eq 2.08E-05 7.51E-09 1.14E-08 0 3.56E-09 4.58E-08 8.42E-09 -1.84E-06
EP-marine kg N eq 8.1E-03 1.12E-05 3.16E-05 0 5.29E-06 2.28E-05 9.05E-06 -2.44E-03
EP-terrestrial mol N eq 8.72E-02 1.24E-04 3.96E-04 0 5.88E-05 4.61E-04 9.94E-05 -2.65E-02
kg NMVOC
POCP 2.53E-02 3.16E-05 8.39E-05 0 1.5E-05 6.32E-05 2.74E-05 -7.93E-03
eq
ADPE kg Sb eq 2.53E-04 1.05E-09 9.2E-10 0 4.98E-10 3.93E-09 4.4E-10 -1.57E-05
ADPF MJ 1.49E+02 4.98E-01 1E-01 0 2.36E-01 2.64E-01 6.43E-02 -5.1E+01
m3 world eq
WDP 9.51E-01 6.88E-05 3.91E-02 0 3.26E-05 5.82E-02 5.14E-04 -7.77E-02
deprived
GWP = Global warming potential; ODP = Depletion potential of the stratospheric ozone layer; AP = Acidification potential of land and water; EP =
Eutrophication potential; POCP = Formation potential of tropospheric ozone photochemical oxidants; ADPE = Abiotic depletion potential for non-fossil
resources; ADPF = Abiotic depletion potential for fossil resources; WDP = Water (user) deprivation potential)
RESULTS OF THE LCA - INDICATORS TO DESCRIBE RESOURCE USE according to EN 15804+A2: 1 door closer
Parameter Unit A1-A3 A4 A5 C1 C2 C3 C4 D
PERE MJ 3.23E+01 1.57E-03 2.65E+00 0 7.43E-04 4.17E-01 8.42E-03 -1.25E+01
PERM MJ 2.98E+00 0 -2.63E+00 0 0 -3.48E-01 0 0
PERT MJ 3.53E+01 1.57E-03 1.84E-02 0 7.43E-04 6.86E-02 8.42E-03 -1.25E+01
PENRE MJ 1.41E+02 4.98E-01 1.87E-01 0 2.36E-01 8.95E+00 6.43E-02 -5.12E+01
PENRM MJ 8.77E+00 0 -8.6E-02 0 0 -8.68E+00 0 0
PENRT MJ 1.5E+02 4.98E-01 1.01E-01 0 2.36E-01 2.64E-01 6.43E-02 -5.12E+01
SM kg 2.03E+00 0 0 0 0 0 0 0
RSF MJ 0 0 0 0 0 0 0 0
NRSF MJ 0 0 0 0 0 0 0 0
FW m3 6.7E-02 2.81E-06 9.2E-04 0 1.33E-06 1.39E-03 1.62E-05 -2.6E-02
PERE = Use of renewable primary energy excluding renewable primary energy resources used as raw materials; PERM = Use of renewable primary
energy resources used as raw materials; PERT = Total use of renewable primary energy resources; PENRE = Use of non-renewable primary energy
excluding non-renewable primary energy resources used as raw materials; PENRM = Use of non-renewable primary energy resources used as raw
materials; PENRT = Total use of non-renewable primary energy resources; SM = Use of secondary material; RSF = Use of renewable secondary fuels;
NRSF = Use of non-renewable secondary fuels; FW = Use of net fresh water
RESULTS OF THE LCA – WASTE CATEGORIES AND OUTPUT FLOWS according to EN 15804+A2:
1 door closer
Parameter Unit A1-A3 A4 A5 C1 C2 C3 C4 D
HWD kg 2.1E-05 4.83E-11 1.54E-10 0 2.29E-11 1.01E-09 9.8E-10 -4.41E-08
NHWD kg 9.03E-01 5.09E-05 1.03E-02 0 2.41E-05 5.91E-02 3.23E-01 -5.5E-01
RWD kg 4.64E-03 5.35E-07 5.25E-06 0 2.53E-07 9.79E-06 7.32E-07 -3.24E-03
CRU kg 0 0 0 0 0 0 0 0
MFR kg 0 0 0 0 0 2.73E+00 0 0
MER kg 0 0 0 0 0 0 0 0
EEE MJ 0 0 4.8E-01 0 0 0 0 0
EET MJ 0 0 8.75E-01 0 0 0 0 0
HWD = Hazardous waste disposed; NHWD = Non-hazardous waste disposed; RWD = Radioactive waste disposed; CRU = Components for re-use;
MFR = Materials for recycling; MER = Materials for energy recovery; EEE = Exported electrical energy; EET = Exported thermal energy
4 Environmental Product Declaration - dormakaba - BEST HD8000
RESULTS OF THE LCA – additional impact categories according to EN 15804+A2-optional:
1 door closer
Parameter Unit A1-A3 A4 A5 C1 C2 C3 C4 D
Disease
PM 4.7E-07 1.85E-10 4.94E-10 0 8.74E-11 1.29E-09 4.35E-10 -2.08E-07
incidence
IR kBq U235 eq 7.5E-01 7.64E-05 8.06E-04 0 3.62E-05 8.82E-04 7.53E-05 -6.73E-01
ETP-fw CTUe 5.64E+01 3.53E-01 4.75E-02 0 1.67E-01 9.9E-02 3.67E-02 -1.51E+01
HTP-c CTUh 8.22E-09 6.63E-12 2.54E-12 0 3.14E-12 8.57E-12 5.44E-12 -4.18E-09
HTP-nc CTUh 1.65E-07 2.84E-10 1.14E-10 0 1.34E-10 8.67E-10 6E-10 -1.19E-08
SQP SQP 5.96E+01 1.28E-03 2.67E-02 0 6.06E-04 7.9E-02 1.34E-02 -2.08E-01
PM = Potential incidence of disease due to PM emissions; IR = Potential Human exposure efficiency relative to U235; ETP-fw = Potential comparative
Toxic Unit for ecosystems; HTP-c = Potential comparative Toxic Unit for humans (cancerogenic); HTP-nc = Potential comparative Toxic Unit for humans
(not cancerogenic); SQP = Potential soil quality index
Disclaimer 1 – for the indicator “Potential Human exposure efficiency relative to U235”. This impact category deals mainly with the
eventual impact of low-dose ionizing radiation on human health of the nuclear fuel cycle. It does not consider effects due to possible
nuclear accidents, occupational exposure or radioactive waste disposal in underground facilities. Potential ionizing radiation from the
soil, radon and from some construction materials is also not measured by this indicator.
Disclaimer 2 – for the indicators “abiotic depletion potential for non-fossil resources”, “abiotic depletion potential for fossil resources”,
“water (user) deprivation potential, deprivation-weighted water consumption”, “potential comparative toxic unit for ecosystems”,
“potential comparative toxic unit for humans – cancerogenic”, “Potential comparative toxic unit for humans - not cancerogenic”,
“potential soil quality index”. The results of this environmental impact indicator shall be used with care as the uncertainties on these
results are high as there is limited experience with the indicator.
References
ADA (version 1-6)
Americans with Disabilities Act 1990 IBU
Institut Bauen und Umwelt e.V.: General Programme
ANSI/ICC A117.1:2017 Instructions for the Preparation of EPDs at the Institut
ANSI/ICC A117.1 - 2009, Accessible and usable buildings and Bauen und Umwelt e.V. Version 1., Berlin: Institut
facilities Bauen und Umwelt e.V., 2016. www.ibu-epd.com
ANSI/BHMA A156.4:2019 GaBi
ANSI/BHMA A156.4 - 2013, Door controls — Closers Sphera Solutions GmbH
Gabi Software System and Database for Life Cycle
Candidate List of REACH Regulation /1907/2006/EC (date: Engineering 1992-2020
16.01.2020) Version 10.0.0.71
University of Stuttgart
ECHA Leinfelden-Echterdingen
European Chemicals Agency: https://echa.europa.eu/de/home
ISO 9001 GaBi ts documentation
Quality Management System: ISO 9001:2015 GaBi life cycle inventory data documentation
(https://www.gabi-software.com/support/gabi/gabidatabase-
ISO 14001 2020-lci-documentation/).
Environmental Management System: ISO 14001:2015
LCA-tool dormakaba
ISO 50001 LCA tool, version 1.0, 2021.
Energy Management System: ISO 50001:2011 UL 10C:2016 Developed by Sphera Solutions GmbH
UL 10C, Positive pressure fire tests of door assemblies
PCR Part A
REACH PCR – Part A: Calculation Rules for the Life Cycle Assessment
Registration, Evaluation, Authorisation and Restriction and Requirements on the Project Re-port
of Chemicals (REACH), Regulation (EC) No 1907/2006 according to EN 15804+A2:2019, Version 1.0, 2020, Institut
Bauen und Umwelt e.V., www.ibu-epd.com.
EN 15804:2019+A2
EN 15804:2019+A2 (in press), Sustainability of PCR Part B
construction works — Environmental Product PCR – Part B: Requirements on the EPD for Building
Declarations — Core rules for the product category of Hardware product, version 1.2, Institut Bauen und
construction products. Umwelt e.V., www.ibu-epd.com, 2017.
Further References
5 Environmental Product Declaration - dormakaba - BEST HD8000
Publisher
Institut Bauen und Umwelt e.V. +49 (0)30 3087748- 0
Hegelplatz 1 info@ibu-epd.com
10117 Berlin www.ibu-epd.com
Germany
Programme holder
Institut Bauen und Umwelt e.V. +49 (0)30 3087748- 0
Hegelplatz 1 info@ibu-epd.com
10117 Berlin www.ibu-epd.com
Germany
Author of the Life Cycle Assessment
Sphera Solutions GmbH +49 711 341817-0
Hauptstraße 111- 113 info@sphera.com
70771 Leinfelden-Echterdingen www.sphera.com
Germany
Owner of the Declaration
dormakaba International Holding GmbH +49 2333 793-0
DORMA Platz 1 info.de@dormakaba.com
58256 Ennepetal www.dormakaba.com
Germany
6 Environmental Product Declaration - dormakaba - BEST HD8000
