ENVIRONMENTAL PRODUCT DECLARATION
as per ISO 14025 and EN 15804+A2
Owner of the Declaration dormakaba International Holding GmbH
Publisher Institut Bauen und Umwelt e.V. (IBU)
Programme holder Institut Bauen und Umwelt e.V. (IBU)
Declaration number EPD-DOR-20220212-CBA1-EN
Issue date 06.09.2022
Valid to 05.09.2027
BEST 47H Mortise Series
dormakaba
www.ibu-epd.com | https://epd-online.com
General Information
dormakaba BEST 47H Mortise Series
Programme holder Owner of the declaration
IBU – Institut Bauen und Umwelt e.V. dormakaba International Holding GmbH
Hegelplatz 1 DORMA Platz 1
10117 Berlin 58256 Ennepetal
Germany Germany
Declaration number Declared product / declared unit
EPD-DOR-20220212-CBA1-EN 1 mortise lock (1 piece) of the BEST 47H Series.
This declaration is based on the product category rules: Scope:
Building Hardware products, 01.08.2021 This Environmental Product Declaration refers to a specific lock
(PCR checked and approved by the SVR) manufactured by dormakaba. The production site is located in Indianapolis
(USA).
Issue date The data represents the year 2020.
The owner of the declaration shall be liable for the underlying information
06.09.2022
and evidence; the IBU shall not be liable with respect to manufacturer
information, life cycle assessment data and evidences.
Valid to
The EPD was created according to the specifications of EN 15804+A2. In
05.09.2027 the following, the standard will be simplified as EN 15804.
Verification
The standard EN 15804 serves as the core PCR
Independent verification of the declaration and data according to ISO
14025:2011
internally X externally
Dipl.-Ing. Hans Peters
(Chairman of Institut Bauen und Umwelt e.V.)
Florian Pronold Dr.-Ing. Wolfram Trinius,
(Managing Director Institut Bauen und Umwelt e.V.) (Independent verifier)
1 Environmental Product Declaration - dormakaba - BEST 47H Mortise Series
Product
Product description/Product definition Base materials/Ancillary materials
BEST's 47H series mortise locks deliver exceptional strength, The major material compositions including the packaging of the
security, and durability. The robust design features and product are listed below:
precision-engineered components make the 47H mortise lock Name Value Unit
series ideal for high traffic applications. Backed by an industry-
Brass 50 %
leading limited lifetime mechanical warranty, the 47H series
Steel 29 %
delivers security you can depend on. For the use and
application of the product the respective national provisions at Stainless steel 11 %
the place of use apply. The standards which can be applied are Electronics 5 %
the following: Zinc 4 %
• ANSI/BHMA A156.13 Plastics 1 %
• ANSI A117.1 (Accessibility, ADA compliant) Other materials <1 %
• Florida Building Code (FBC) listed
The product/s include/s partial articles which contain
• Miami-Dade County Code compliant
substances listed in the Candidate List of REACH Regulation
• UL listed
1907/2006/EC (date: 17.01.2022) exceeding 0.1 percentage by
Application mass: yes
The 47H Mortise Series can be used for following building • Lead (Pb): 7439-92-1 (CAS-No.) is included in some of
types: the alloys used. The concentration of lead in each
• Learning and higher education individual alloy does not exceed 4.0% (by mass).
• Healthcare The Candidate List can be found on the ECHA website
• Government address: https://echa.europa.eu/de/home.
• Retail and commercial
Reference service life
Technical Data The reference service life of the 47H Mortise Series lock
The lock has following technical properties: depends on the traffic pattern and degree of usage of the door.
These locks are rated to ANSI Grade 1, meaning they are
designed to withstand a minimum of 1,000,000 cycles.
However, the 47H Mortise lock has been independently tested
to surpass 10,000,000 cycles.
Performance data of the product with respect to its
characteristics in accordance with the relevant technical
provision which can be applied are mentioned above.
LCA: Calculation rules
Production - Module A1-A3
Declared Unit The product stage includes:
The declared unit is 1 piece of the product: BEST 47H Mortise — A1, raw material extraction, processing and mechanical
Series. treatments, processing of secondary material input (e.g.
Declared unit recycling processes), — A2, transport to the manufacturer,
— A3, manufacturing and assembly including provision of all
Name Value Unit
materials, products and energy, as well as waste processing up
Declared unit 1 piece/product
to the end-of waste state.
Mass of declared Product 3.8 kg
Construction stage - Modules A4-A5
System boundary The construction process stage includes:
The type of EPD is: cradle to gate with options, modules C1– — A4, transport to the building site;
C4, and module D (A1–A3 + C + D and additional modules: A4 — A5, installation into the building;
+ A5) including provision of all materials, products and energy, as well
as waste processing up to the end-of waste state or disposal of
final residues during the construction process stage.
2 Environmental Product Declaration - dormakaba - BEST 47H Mortise Series
End-of-life stage– Modules C1-C4 and D Geographic Representativeness
The end-of-life stage includes: Land or region, in which the declared product system is
— C1, de-construction, demolition: manufactured, used or handled at the end of the product´s
— C2, transport to waste processing; lifespan: United States
— C3, waste processing for reuse, recovery and/or recycling;
— C4, disposal;
Comparability
including provision and all transport, provision of all materials,
Basically, a comparison or an evaluation of EPD data is only
products and related energy and water use.
possible if all the data sets to be compared were created
according to EN 15804 and the building context, respectively
Module D (Benefits and loads beyond the system boundary)
the product-specific characteristics of performance, are taken
includes:
into account.
— D, recycling potentials, expressed as net impacts and
benefits.
LCA: Scenarios and additional technical information
Operational energy use (B6)
Characteristic product properties of biogenic carbon
Name Value Unit
Information on describing the biogenic Carbon Content at
Electricity consumption for 1 year 28.47 kWh
factory gate
Power consumption "on mode" 78 W
Name ValueUnit
Hours per day in use "on mode" 1 h
kg
Biogenic carbon content in product - C Power consumption "standby mode" 0 W
Biogenic carbon content in accompanying kg Hours per day in use "standby mode" 23 h
-
packaging C
End of life (C1-C4)
Note: 1 kg of biogenic carbon is equivalent to 44/12 kg of CO 2. C1: The product dismantling from the building is done manually
without environmental burden.
C2: Transport to waste treatment at end of life is 50km.
Additional technical information for the declared modules.
Name Value Unit
Transport to the building site (A4) Collected separately waste type 3.8 kg
Name Value Unit Recycling 3.58 kg
Litres of fuel per 1 kg (truck) 0.00276l/100km Energy recovery 0.024 kg
Transport distance (truck) 1500 km Final desposition 0,201 kg
Capacity utilisation (including empty runs)
55 % Reuse, recovery and/or recycling potentials (D), relevant
average
scenario information
Transport distance (ship) 10000 km
Name Value Unit
Installation into the building (A5) Recycling 100 %
Name Value Unit
Collection rate is 100%.
Output substances following waste treatment on
0.00017 kg
site (packaging)
3 Environmental Product Declaration - dormakaba - BEST 47H Mortise Series
LCA: Results
Disclaimer:
EP-freshwater: This indicator has been calculated as 'kg P eq' as required in the characterization model (EUTREND model, Struijs et
al., 2009b, as implemented in ReCiPe; http://eplca.jrc.ec.europa.eu/LCDN/developerEF.xhtml)
DESCRIPTION OF THE SYSTEM BOUNDARY (X = INCLUDED IN LCA; MND = MODULE OR INDICATOR NOT DECLARED; MNR
= MODULE NOT RELEVANT)
Benefits and
Construction loads beyond
Product stage Use stage End of life stage
process stage the system
boundaries
la ire ta m w a Ry lp p u s tro p s n a rT g n iru tc a fu n a M e h t m o rf tro p s n a rTe tis e h t o t e ta g y lb m e s s A e s U e c n a n e tn ia M ria p e R tn e m e c a lp e R tn e m h s ib ru fe R y g re n e la n o ita re p Oe s u re ta w la n o ita re p Oe s u n o itc u rts n o c -e Dn o itilo m e d tro p s n a rT g n is s e c o rp e ts a W la s o p s iD -e s u e R-y re v o c e R-g n ilc y c e Rla itn e to p
A1 A2 A3 A4 A5 B1 B2 B3 B4 B5 B6 B7 C1 C2 C3 C4 D
X X X X X MND MND MNR MNR MNR MND MND X X X X X
RESULTS OF THE LCA - ENVIRONMENTAL IMPACT according to EN 15804+A2: 1 mortise lock
Parameter Unit A1-A3 A4 A5 C1 C2 C3 C4 D
GWP-total kg CO 2 eq 9.94E+00 6.23E-01 2.41E-04 0 1.7E-02 6.3E-02 3E-03 -3.28E+00
GWP-fossil kg CO 2 eq 9.87E+00 6.01E-01 6.04E-06 0 1.6E-02 6.3E-02 3E-03 -3.29E+00
GWP-biogenic kg CO 2 eq 5.3E-02 2.2E-02 2.35E-04 0 7.32E-04 1.47E-06 1.04E-05 6E-03
GWP-luluc kg CO 2 eq 1.15E-02 1.39E-05 3.97E-09 0 3.77E-07 3.58E-06 8.78E-06 -3E-03
ODP kg CFC11 eq 1.03E-11 6.21E-17 4.34E-20 0 1.67E-18 3.19E-17 1.13E-17 -2.37E-15
AP mol H+ eq 5.2E-02 5E-03 6.75E-08 0 1.58E-05 1.13E-05 2.19E-05 -1E-02
EP-freshwater kg P eq 1.45E-05 1.3E-07 8.5E-12 0 3.39E-09 5.09E-09 5.24E-09 -2.95E-06
EP-marine kg N eq 7.25E-03 1E-03 2.44E-08 0 5.04E-06 2.54E-06 5.63E-06 -2E-03
EP-terrestrial mol N eq 7.5E-02 1.5E-02 3.04E-07 0 5.6E-05 5.13E-05 6.19E-05 -2E-02
kg NMVOC
POCP 2.17E-02 4E-03 6.46E-08 0 1.43E-05 7.03E-06 1.71E-05 -6E-03
eq
ADPE kg Sb eq 2.04E-03 1.75E-08 6.86E-13 0 4.75E-10 4.38E-10 2.74E-10 3.22E-05
ADPF MJ 1.23E+02 8.27E+00 7.61E-05 0 2.24E-01 2.9E-02 4E-02 -3.57E+01
m3 world eq
WDP 2.15E+00 1E-03 2.99E-05 0 3.1E-05 6E-03 3.2E-04 -8.24E-01
deprived
GWP = Global warming potential; ODP = Depletion potential of the stratospheric ozone layer; AP = Acidification potential of land and water; EP =
Eutrophication potential; POCP = Formation potential of tropospheric ozone photochemical oxidants; ADPE = Abiotic depletion potential for non-fossil
resources; ADPF = Abiotic depletion potential for fossil resources; WDP = Water (user) deprivation potential)
RESULTS OF THE LCA - INDICATORS TO DESCRIBE RESOURCE USE according to EN 15804+A2: 1 mortise lock
Parameter Unit A1-A3 A4 A5 C1 C2 C3 C4 D
PERE MJ 2.48E+01 2.6E-02 2E-03 0 7.08E-04 2.1E-02 5E-03 -4.26E+00
PERM MJ 1.5E-02 0 -2E-03 0 0 -1.3E-02 0 0
PERT MJ 2.48E+01 2.6E-02 1.38E-05 0 7.08E-04 8E-03 5E-03 -4.26E+00
PENRE MJ 1.22E+02 8.28E+00 7.61E-05 0 2.25E-01 8.41E-01 4E-02 -3.58E+01
PENRM MJ 8.11E-01 0 0 0 0 -8.11E-01 0 0
PENRT MJ 1.23E+02 8.28E+00 7.61E-05 0 2.25E-01 2.9E-02 4E-02 -3.58E+01
SM kg 2.61E+00 0 0 0 0 0 0 0
RSF MJ 0 0 0 0 0 0 0 0
NRSF MJ 0 0 0 0 0 0 0 0
FW m3 6.91E-02 4.72E-05 7.04E-07 0 1.27E-06 1.55E-04 1.01E-05 -3.3E-02
PERE = Use of renewable primary energy excluding renewable primary energy resources used as raw materials; PERM = Use of renewable primary
energy resources used as raw materials; PERT = Total use of renewable primary energy resources; PENRE = Use of non-renewable primary energy
excluding non-renewable primary energy resources used as raw materials; PENRM = Use of non-renewable primary energy resources used as raw
materials; PENRT = Total use of non-renewable primary energy resources; SM = Use of secondary material; RSF = Use of renewable secondary fuels;
NRSF = Use of non-renewable secondary fuels; FW = Use of net fresh water
RESULTS OF THE LCA – WASTE CATEGORIES AND OUTPUT FLOWS according to EN 15804+A2:
1 mortise lock
Parameter Unit A1-A3 A4 A5 C1 C2 C3 C4 D
HWD kg 3.79E-07 8.05E-10 1.12E-13 0 2.18E-11 1.12E-10 6.1E-10 -1.57E-06
NHWD kg 9.16E-01 8.47E-04 7.55E-06 0 2.3E-05 7E-03 2.01E-01 -1.9E-02
RWD kg 4.97E-03 8.95E-06 4E-09 0 2.41E-07 1.09E-06 4.56E-07 -2.93E-04
CRU kg 0 0 0 0 0 0 0 0
MFR kg 0 0 0 0 0 3.56E+00 0 0
MER kg 0 0 0 0 0 0 0 0
4 Environmental Product Declaration - dormakaba - BEST 47H Mortise Series
EEE MJ 1.7E-02 0 3.65E-04 0 0 0 0 0
EET MJ 3.1E-02 0 6.61E-04 0 0 0 0 0
HWD = Hazardous waste disposed; NHWD = Non-hazardous waste disposed; RWD = Radioactive waste disposed; CRU = Components for re-use;
MFR = Materials for recycling; MER = Materials for energy recovery; EEE = Exported electrical energy; EET = Exported thermal energy
RESULTS OF THE LCA – additional impact categories according to EN 15804+A2-optional:
1 mortise lock
Parameter Unit A1-A3 A4 A5 C1 C2 C3 C4 D
Disease
PM 5.96E-07 8.08E-08 3.74E-13 0 8.33E-11 1.44E-10 2.71E-10 -2.07E-07
incidence
IR kBq U235 eq 6.77E-01 1E-03 6.19E-07 0 3.45E-05 9.81E-05 4.69E-05 -2.3E-02
ETP-fw CTUe 6.6E+01 5.86E+00 3.61E-05 0 1.59E-01 1.1E-02 2.3E-02 -1.1E+01
HTP-c CTUh 5.9E-07 1.1E-10 1.91E-15 0 2.99E-12 9.53E-13 3.39E-12 -1.4E-09
HTP-nc CTUh 2.46E-07 4.81E-09 8.28E-14 0 1.28E-10 9.65E-11 3.74E-10 2.03E-07
SQP SQP 2.83E+01 2.1E-02 2.02E-05 0 5.77E-04 9E-03 8E-03 -1.47E+00
PM = Potential incidence of disease due to PM emissions; IR = Potential Human exposure efficiency relative to U235; ETP-fw = Potential comparative
Toxic Unit for ecosystems; HTP-c = Potential comparative Toxic Unit for humans (cancerogenic); HTP-nc = Potential comparative Toxic Unit for humans
(not cancerogenic); SQP = Potential soil quality index
Disclaimer 1 – for the indicator “Potential Human exposure efficiency relative to U235”. This impact category deals mainly with the
eventual impact of low-dose ionizing radiation on human health of the nuclear fuel cycle. It does not consider effects due to possible
nuclear accidents, occupational exposure or radioactive waste disposal in underground facilities. Potential ionizing radiation from the
soil, radon and from some construction materials is also not measured by this indicator.
Disclaimer 2 – for the indicators “abiotic depletion potential for non-fossil resources”, “abiotic depletion potential for fossil resources”,
“water (user) deprivation potential, deprivation-weighted water consumption”, “potential comparative toxic unit for ecosystems”,
“potential comparative toxic unit for humans – cancerogenic”, “Potential comparative toxic unit for humans - not cancerogenic”,
“potential soil quality index”. The results of this environmental impact indicator shall be used with care as the uncertainties on these
results are high as there is limited experience with the indicator.
References
ADA (version 1-6) GaBi
Americans with Disabilities Act 1990. Sphera Solutions GmbH
Gabi Software System and Database for Life Cycle Engineering
ANSI A117.1 1992-2020 Version 10.0.0.71 University of StuttgartLeinfelden-
ANSI A117.1-2017: Accessible and Usable Buildings. Echterdingen.
ANSI/BHMA A156.13 GaBi ts documentation
ANSI/BHMA A1564.13:2017 - Mortise Locks. GaBi life cycle inventory data documentation (https://www.gabi-
software.com/support/gabi/gabidatabase-2020-lci-
EN 15804 documentation/).
EN 15804:2019+A2, Sustainability of construction works —
Environmental Product Declarations — Core rules for the LCA-tool dormakaba
product category of construction products. LCA-tool, IBU-DOR-202104-LT1-EN.
Developed by Sphera Solutions GmbH.
REACH Regulation 1907/2006/EC
Regulation (EC) No 1907/2006 of the European Parliament and Miami-Dade County Code
of the Council on the Registration, Evaluation, Authorisation https://www.miamidade.gov/cob/ordinances-enacted-by-
and Restriction of Chemicals (REACH). bcc.asp.
Further References PCR Part A
PCR – Part A: Calculation Rules for the Life Cycle Assessment
Florida Building Code and Requirements on the Project Re-port according to EN
https://floridabuilding.org/c/default.aspx. 15804+A2:2019, Version 1.0, 2020, Institut Bauen und Umwelt
e.V., www.ibu-epd.com.
IBU 2021
Institut Bauen und Umwelt e.V.: General Instructions for the PCR Part B
EPDs programme of Institut Bauen und Umwelt e.V. Version PCR – Part B: Requirements on the EPD for Building Hardware
2.0., Berlin: Institut Bauen und Umwelt e.V., 2021. www.ibu- product, version 1.2, Institut Bauen und Umwelt e.V., www.ibu-
epd.com. epd.com, 2017.
UL
Underwriters Laboratories, https://www.ul.com/.
5 Environmental Product Declaration - dormakaba - BEST 47H Mortise Series
Publisher
Institut Bauen und Umwelt e.V. +49 (0)30 3087748- 0
Hegelplatz 1 info@ibu-epd.com
10117 Berlin www.ibu-epd.com
Germany
Programme holder
Institut Bauen und Umwelt e.V. +49 (0)30 3087748- 0
Hegelplatz 1 info@ibu-epd.com
10117 Berlin www.ibu-epd.com
Germany
Author of the Life Cycle Assessment
Sphera Solutions GmbH +49 711 341817-0
Hauptstraße 111- 113 info@sphera.com
70771 Leinfelden-Echterdingen www.sphera.com
Germany
Owner of the Declaration
dormakaba International Holding GmbH +49 2333 793-0
DORMA Platz 1 info.de@dormakaba.com
58256 Ennepetal www.dormakaba.com
Germany
6 Environmental Product Declaration - dormakaba - BEST 47H Mortise Series
