ENVIRONMENTAL PRODUCT DECLARATION
as per ISO 14025 and EN 15804+A2
Owner of the Declaration dormakaba International Holding GmbH
Publisher Institut Bauen und Umwelt e.V. (IBU)
Programme holder Institut Bauen und Umwelt e.V. (IBU)
Declaration number EPD-DOR-20210303-CBA1-EN
Issue date 04.05.2022
Valid to 03.05.2027
BEST 1E Series
dormakaba
www.ibu-epd.com | https://epd-online.com
General Information
dormakaba BEST 1E Series
Programme holder Owner of the declaration
IBU – Institut Bauen und Umwelt e.V. dormakaba International Holding GmbH
Hegelplatz 1 DORMA Platz 1
10117 Berlin 58256 Ennepetal
Germany Germany
Declaration number Declared product / declared unit
EPD-DOR-20210303-CBA1-EN 1 cylinder (1 piece) of the BEST 1E Series.
This declaration is based on the product category rules: Scope:
Building Hardware products, 01.08.2021 This Environmental Product Declaration refers to a specific cylinder
(PCR checked and approved by the SVR) manufactured by dormakaba. The production site is located in Indianapolis
(USA).
Issue date The data represents the year 2020.
The owner of the declaration shall be liable for the underlying information
04.05.2022
and evidence; the IBU shall not be liable with respect to manufacturer
information, life cycle assessment data and evidences.
Valid to
The EPD was created according to the specifications of EN 15804+A2. In
03.05.2027 the following, the standard will be simplified as EN 15804.
Verification
The standard EN 15804 serves as the core PCR
Independent verification of the declaration and data according to ISO
14025:2011
internally X externally
Dipl.-Ing. Hans Peters
(Chairman of Institut Bauen und Umwelt e.V.)
Florian Pronold Dr.-Ing. Wolfram Trinius,
(Managing Director Institut Bauen und Umwelt e.V.) (Independent verifier)
1 Environmental Product Declaration - dormakaba - BEST 1E Series
Product
provision:
Product description/Product definition
BEST mortise and rim cylinders may be altered to function with
• ANSI/BHMA Grade 1
other manufacturers' locks by use of different cams and
different cylinder rings. Special cylinder variations are available Base materials/Ancillary materials
for most applications. BEST cylinders are machined from brass
Name Value Unit
or bronze bar stock and are available in a variety of finishes.
Brass 41 %
For the use and application of the product the respective
national provisions at the place of use apply. The standards Steel 26 %
which can be applied are the following: Stainless steel 27 %
• ANSI/BHMA Grade 1 Paper 5 %
• UL listed Others <1 %
Application The product/s include/s partial articles which contain
substances listed in the Candidate List of REACH Regulation
The BEST 1E Series can be used in following building types:
1907/2006/EC (date: 17.01.2022) exceeding 0.1 percentage by
• Learning and higher education
mass: yes
• Healthcare
• Lead (Pb): 7439-92-1 (CAS-No.) is included in some of
• Government
the alloys used. The concentration of lead in each
• Retail and commercial
individual alloy does not exceed 4.0% (by mass).
Technical Data The Candidate List can be found on the ECHA website
The cylinder has following technical properties: address: https://echa.europa.eu/de/home.
• Cylinder diameter: 1-5/32" Reference service life
• How to order example: 1E74-C4-RP3-626
The reference service life of the BEST 1E Series depends on
• Products covered by on or more of the following
the traffic pattern and degree of usage of the cylinder.
patents: 5,590,555 5,794,472
BESTcylinders are certified to BHMA/ANSI Grade 1, meaning
The performance data of the product with respect to its
they are designed to withstand a minimum of 40,000 uses.
characteristics are in accordance with the relevant technical
LCA: Calculation rules
End-of-life stage– Modules C1-C4 and D
Declared Unit The end-of-life stage includes:
The declared unit is 1 piece of the product: BEST 1E Series. — C1, de-construction, demolition:
Declared unit — C2, transport to waste processing;
— C3, waste processing for reuse, recovery and/or recycling;
Name Value Unit
— C4, disposal;
Declared unit 1 piece/product
including provision and all transport, provision of all materials,
Mass of declared Product 0.26 kg products and related energy and water use.
System boundary Module D (Benefits and loads beyond the system boundary)
The type of EPD is: cradle to gate with options, modules C1– includes:
C4, and module D (A1–A3 + C + D and additional modules: A4 — D, recycling potentials, expressed as net impacts and
+ A5) benefits.
Geographic Representativeness
Production - Module A1-A3
Land or region, in which the declared product system is
The product stage includes:
manufactured, used or handled at the end of the product´s
— A1, raw material extraction, processing and mechanical
lifespan: North America
treatments, processing of secondary material input (e.g.
recycling processes), — A2, transport to the manufacturer,
— A3, manufacturing and assembly including provision of all
Comparability
materials, products and energy, as well as waste processing up
Basically, a comparison or an evaluation of EPD data is only
to the end-of waste state.
possible if all the data sets to be compared were created
according to EN 15804 and the building context, respectively
Construction stage - Modules A4-A5
the product-specific characteristics of performance, are taken
The construction process stage includes:
into account.
— A4, transport to the building site;
— A5, installation into the building;
including provision of all materials, products and energy, as well
as waste processing up to the end-of waste state or disposal of
final residues during the construction process stage.
2 Environmental Product Declaration - dormakaba - BEST 1E Series
LCA: Scenarios and additional technical information
Installation into the building (A5)
Characteristic product properties of biogenic carbon
Name Value Unit
Information on describing the biogenic Carbon Content at
Output substances following waste treatment on
factory gate 0.01417 kg
site (packaging)
Name ValueUnit
Biogenic carbon content in accompanying kg End of life (C1-C4)
0.01
packaging C C1: The product dismantling from the building is done manually
without environmental burden.
Note: 1 kg of biogenic carbon is equivalent to 44/12 kg of CO .
2 C2: Transport to waste treatment at end of life is 50km.
Name Value Unit
Additional technical information for the declared modules. Collected separately waste type 0.25 kg
Transport to the building site (A4) Recycling 0.249 kg
Energy recovery 0.0006 kg
Name Value Unit
Final deposition 0,0001 kg
Litres of fuel per 1 kg (truck) 0.00276l/100km
Transport distance (truck) 1500 km Region for end of life: Global
Capacity utilisation (including empty runs)
55 %
average Reuse, recovery and/or recycling potentials (D), relevant
Transport distance (ship) 10000 km scenario information
Name Value Unit
Collection rate is 100%.
3 Environmental Product Declaration - dormakaba - BEST 1E Series
LCA: Results
Disclaimer:
EP-freshwater: This indicator has been calculated as 'kg P eq' as required in the characterization model (EUTREND model, Struijs et
al., 2009b, as implemented in ReCiPe; http://eplca.jrc.ec.europa.eu/LCDN/developerEF.xhtml)
DESCRIPTION OF THE SYSTEM BOUNDARY (X = INCLUDED IN LCA; MND = MODULE OR INDICATOR NOT DECLARED; MNR
= MODULE NOT RELEVANT)
Benefits and
Construction loads beyond
Product stage Use stage End of life stage
process stage the system
boundaries
la ire ta m w a Ry lp p u s tro p s n a rT g n iru tc a fu n a M e h t m o rf tro p s n a rTe tis e h t o t e ta g y lb m e s s A e s U e c n a n e tn ia M ria p e R tn e m e c a lp e R tn e m h s ib ru fe R y g re n e la n o ita re p Oe s u re ta w la n o ita re p Oe s u n o itc u rts n o c -e Dn o itilo m e d tro p s n a rT g n is s e c o rp e ts a W la s o p s iD -e s u e R-y re v o c e R-g n ilc y c e Rla itn e to p
A1 A2 A3 A4 A5 B1 B2 B3 B4 B5 B6 B7 C1 C2 C3 C4 D
X X X X X MND MND MNR MNR MNR MND MND X X X X X
RESULTS OF THE LCA - ENVIRONMENTAL IMPACT according to EN 15804+A2: 1 cylindrical lock
Parameter Unit A1-A3 A4 A5 C1 C2 C3 C4 D
GWP-total kg CO 2 eq 1.06E+01 3.67E-02 3.16E-01 0 1.74E-02 5.69E-01 4.93E-03 -4.63E+00
GWP-fossil kg CO 2 eq 1.1E+01 3.51E-02 1.29E-02 0 1.66E-02 5.69E-01 4.9E-03 -4.62E+00
GWP-biogenic kg CO 2 eq -3.83E-01 1.62E-03 3.03E-01 0 7.68E-04 1.33E-05 1.67E-05 -5.4E-03
GWP-luluc kg CO 2 eq 9.93E-03 8.35E-07 5.4E-06 0 3.96E-07 3.22E-05 1.41E-05 -5.52E-04
ODP kg CFC11 eq 5.76E-10 3.7E-18 5.86E-17 0 1.75E-18 2.87E-16 1.82E-17 -1.54E-11
AP mol H+ eq 4.13E-02 3.51E-05 8.8E-05 0 1.66E-05 1.01E-04 3.51E-05 -1.43E-02
EP-freshwater kg P eq 2.08E-05 7.51E-09 1.14E-08 0 3.56E-09 4.58E-08 8.42E-09 -1.84E-06
EP-marine kg N eq 8.1E-03 1.12E-05 3.16E-05 0 5.29E-06 2.28E-05 9.05E-06 -2.44E-03
EP-terrestrial mol N eq 8.72E-02 1.24E-04 3.96E-04 0 5.88E-05 4.61E-04 9.94E-05 -2.65E-02
kg NMVOC
POCP 2.53E-02 3.16E-05 8.39E-05 0 1.5E-05 6.32E-05 2.74E-05 -7.93E-03
eq
ADPE kg Sb eq 2.53E-04 1.05E-09 9.2E-10 0 4.98E-10 3.93E-09 4.4E-10 -1.57E-05
ADPF MJ 1.49E+02 4.98E-01 1E-01 0 2.36E-01 2.64E-01 6.43E-02 -5.1E+01
m3 world eq
WDP 9.51E-01 6.88E-05 3.91E-02 0 3.26E-05 5.82E-02 5.14E-04 -7.77E-02
deprived
GWP = Global warming potential; ODP = Depletion potential of the stratospheric ozone layer; AP = Acidification potential of land and water; EP =
Eutrophication potential; POCP = Formation potential of tropospheric ozone photochemical oxidants; ADPE = Abiotic depletion potential for non-fossil
resources; ADPF = Abiotic depletion potential for fossil resources; WDP = Water (user) deprivation potential)
RESULTS OF THE LCA - INDICATORS TO DESCRIBE RESOURCE USE according to EN 15804+A2: 1 cylindrical lock
Parameter Unit A1-A3 A4 A5 C1 C2 C3 C4 D
PERE MJ 3.23E+01 1.57E-03 2.65E+00 0 7.43E-04 4.17E-01 8.42E-03 -1.25E+01
PERM MJ 2.98E+00 0 -2.63E+00 0 0 -3.48E-01 0 0
PERT MJ 3.53E+01 1.57E-03 1.84E-02 0 7.43E-04 6.86E-02 8.42E-03 -1.25E+01
PENRE MJ 1.41E+02 4.98E-01 1.87E-01 0 2.36E-01 8.95E+00 6.43E-02 -5.12E+01
PENRM MJ 8.77E+00 0 -8.6E-02 0 0 -8.68E+00 0 0
PENRT MJ 1.5E+02 4.98E-01 1.01E-01 0 2.36E-01 2.64E-01 6.43E-02 -5.12E+01
SM kg 2.03E+00 0 0 0 0 0 0 0
RSF MJ 0 0 0 0 0 0 0 0
NRSF MJ 0 0 0 0 0 0 0 0
FW m3 6.7E-02 2.81E-06 9.2E-04 0 1.33E-06 1.39E-03 1.62E-05 -2.6E-02
PERE = Use of renewable primary energy excluding renewable primary energy resources used as raw materials; PERM = Use of renewable primary
energy resources used as raw materials; PERT = Total use of renewable primary energy resources; PENRE = Use of non-renewable primary energy
excluding non-renewable primary energy resources used as raw materials; PENRM = Use of non-renewable primary energy resources used as raw
materials; PENRT = Total use of non-renewable primary energy resources; SM = Use of secondary material; RSF = Use of renewable secondary fuels;
NRSF = Use of non-renewable secondary fuels; FW = Use of net fresh water
RESULTS OF THE LCA – WASTE CATEGORIES AND OUTPUT FLOWS according to EN 15804+A2:
1 cylindrical lock
Parameter Unit A1-A3 A4 A5 C1 C2 C3 C4 D
HWD kg 2.1E-05 4.83E-11 1.54E-10 0 2.29E-11 1.01E-09 9.8E-10 -4.41E-08
NHWD kg 9.03E-01 5.09E-05 1.03E-02 0 2.41E-05 5.91E-02 3.23E-01 -5.5E-01
RWD kg 4.64E-03 5.35E-07 5.25E-06 0 2.53E-07 9.79E-06 7.32E-07 -3.24E-03
CRU kg 0 0 0 0 0 0 0 0
MFR kg 0 0 0 0 0 2.73E+00 0 0
MER kg 0 0 0 0 0 0 0 0
4 Environmental Product Declaration - dormakaba - BEST 1E Series
EEE MJ 0 0 4.8E-01 0 0 0 0 0
EET MJ 0 0 8.75E-01 0 0 0 0 0
HWD = Hazardous waste disposed; NHWD = Non-hazardous waste disposed; RWD = Radioactive waste disposed; CRU = Components for re-use;
MFR = Materials for recycling; MER = Materials for energy recovery; EEE = Exported electrical energy; EET = Exported thermal energy
RESULTS OF THE LCA – additional impact categories according to EN 15804+A2-optional:
1 cylindrical lock
Parameter Unit A1-A3 A4 A5 C1 C2 C3 C4 D
Disease
PM 4.7E-07 1.85E-10 4.94E-10 0 8.74E-11 1.29E-09 4.35E-10 -2.08E-07
incidence
IR kBq U235 eq 7.5E-01 7.64E-05 8.06E-04 0 3.62E-05 8.82E-04 7.53E-05 -6.73E-01
ETP-fw CTUe 5.64E+01 3.53E-01 4.75E-02 0 1.67E-01 9.9E-02 3.67E-02 -1.51E+01
HTP-c CTUh 8.22E-09 6.63E-12 2.54E-12 0 3.14E-12 8.57E-12 5.44E-12 -4.18E-09
HTP-nc CTUh 1.65E-07 2.84E-10 1.14E-10 0 1.34E-10 8.67E-10 6E-10 -1.19E-08
SQP SQP 5.96E+01 1.28E-03 2.67E-02 0 6.06E-04 7.9E-02 1.34E-02 -2.08E-01
PM = Potential incidence of disease due to PM emissions; IR = Potential Human exposure efficiency relative to U235; ETP-fw = Potential comparative
Toxic Unit for ecosystems; HTP-c = Potential comparative Toxic Unit for humans (cancerogenic); HTP-nc = Potential comparative Toxic Unit for humans
(not cancerogenic); SQP = Potential soil quality index
Disclaimer 1 – for the indicator “Potential Human exposure efficiency relative to U235”. This impact category deals mainly with the
eventual impact of low-dose ionizing radiation on human health of the nuclear fuel cycle. It does not consider effects due to possible
nuclear accidents, occupational exposure or radioactive waste disposal in underground facilities. Potential ionizing radiation from the
soil, radon and from some construction materials is also not measured by this indicator.
Disclaimer 2 – for the indicators “abiotic depletion potential for non-fossil resources”, “abiotic depletion potential for fossil resources”,
“water (user) deprivation potential, deprivation-weighted water consumption”, “potential comparative toxic unit for ecosystems”,
“potential comparative toxic unit for humans – cancerogenic”, “Potential comparative toxic unit for humans - not cancerogenic”,
“potential soil quality index”. The results of this environmental impact indicator shall be used with care as the uncertainties on these
results are high as there is limited experience with the indicator.
References
Standards
GaBi ts documentation
ISO 14025 GaBi life cycle inventory data documentation (https://www.gabi-
DIN EN ISO 14025:2011-10, Environmental labels and software.com/support/gabi/gabidatabase- 2020-lci-
declarations — Type III environmental declarations — documentation/).
Principles and procedures.
LCA-tool dormakaba
Registration, Evaluation, Authorisation and Restriction of LCA tool, IBU-DOR-202104-LT1-EN.
Chemicals (REACH) Developed by Sphera Solutions GmbH.
Regulation (EC) No 1907/2006 of the European Parliament and
of the Council on the Registration, Evaluation, Authorisation PCR Part A
and Restriction of Chemicals (REACH). PCR – Part A: Calculation Rules for the Life Cycle Assessment
and Requirements on the Project Re-port according to EN
Further References 15804+A2:2019, Version 1.0, Institut Bauen und Umwelt e.V.,
www.ibu-epd.com.
American National Standards Institute (ANSI).
PCR Part B
Builders Hardware Manufacturers Association (BHMA). PCR – Part B: Requirements on the EPD for Building Hardware
product, version 1.3, Institut Bauen und Umwelt e.V., www.ibu-
IBU epd.com, 2019.
Institut Bauen und Umwelt e.V.: General Instructions for the
EPDs programme of Institut Bauen und Umwelt e.V. Version Underwriters Laboratories (UL).
2.0., Berlin: Institut Bauen und Umwelt e.V., 2021. www.ibu-
epd.com.
GaBi ts software
Sphera Solutions GmbH Gabi Software System and Database
for Life Cycle Engineering 1992-2020 Version 10.0.0.71
University of Stuttgart Leinfelden-Echterdingen.
5 Environmental Product Declaration - dormakaba - BEST 1E Series
Publisher
Institut Bauen und Umwelt e.V. +49 (0)30 3087748- 0
Hegelplatz 1 info@ibu-epd.com
10117 Berlin www.ibu-epd.com
Germany
Programme holder
Institut Bauen und Umwelt e.V. +49 (0)30 3087748- 0
Hegelplatz 1 info@ibu-epd.com
10117 Berlin www.ibu-epd.com
Germany
Author of the Life Cycle Assessment
Sphera Solutions GmbH +49 711 341817-0
Hauptstraße 111- 113 info@sphera.com
70771 Leinfelden-Echterdingen www.sphera.com
Germany
Owner of the Declaration
dormakaba International Holding GmbH +49 2333 793-0
DORMA Platz 1 info.de@dormakaba.com
58256 Ennepetal www.dormakaba.com
Germany
6 Environmental Product Declaration - dormakaba - BEST 1E Series
