ver2 2015
ENVIRONMENTAL PRODUCT DECLARATION
in accordance with ISO 14025, ISO 21930 and EN 15804
Owner of the declaration: BEWI ASA
Program operator: The Norwegian EPD Foundation
Publisher: The Norwegian EPD Foundation
Declaration number: NEPD-2796-1492-EN
Registration number: NEPD-2796-1492-EN
ECO Platform reference number: -
Issue date: 27.04.2021
Valid to: 27.04.2026
BEWi EPS 80
EPS Insulation boards
BEWI ASA
www.epd-norge.no
NEPD-2796-1492-EN BEWi EPS 80 EPS Insulation boards (ver1)
General information
Product Owner of the declaration
BEWi EPS 80 BEWI ASA
Contact person: Trude Brustad
Phone: +47 99 20 93 27
e-mail: trude.brustad@bewi.com
Program operator Manufacturer
The Norwegian EPD Foundation BEWI ASA
Post Box 5250 Majorstuen, 0303 Oslo, Norway Hamarvikringen 64, 7263 Hamarvik
Phone: (+47) 23 08 80 00 Phone: +47 72 44 88 88
e-mail: post@epd-norge.no e-mail: ordre@bewi.com
Declaration number Place of production
NEPD-2796-1492-EN Norway
ECO Platform reference number Management system
-
Product Category Rules Organisation number
EN 15804:2012 + A1:2013 serves as core PCR 910,209,205
NPCR 012:2018 Part B for Thermal insulation products
Statement of liability Issue date
The owner of the declaration shall be liable for the 27.04.2021
underlying information and evidence. EPD Norway shall
not be liable with respect to manufacturerinformation, life
cycle assessment data and evidences.
Valid to
27.04.2026
Declared unit Year of study
- 2020
Declared unit with option (A1-A3, A4, C1-C4, D) Comparability
1 m² EPS insulation board with 38 mm thickness at R=1 m² EPD of construction products may not be comparable if they
K/W, transportation to site, waste handling and recovery. not comply with EN 15804 and seen in a building context.
Functional unit The EPD has been worked out by
- Michael M. Jenssen, Asplan Viak AS
Verification
The CEN Norm EN 15804 serves as the core PCR.
Independent verification of the declaration and data,
according to ISO14025:2010
internal external
Approved
Third party verifier:
Jane Anderson, ConstructionLCA Ltd
Independent verifier approved by EPD Norway
NEPD-2796-1492-EN BEWi EPS 80 EPS Insulation boards (ver1)
2/7
Product
Product variation and calculation of averages
The insulation board is provided in several dimensions and thicknesses. Please use the conversion table below for other sizes
than the declared unit.
No variation between sites; single production site declared.
Product description
Expanded polystyrene (EPS) is a common material used for thermal insulation of buildings, including floors, walls and ceilings. It
is a polymer foam, consisting of air-filled polystyrene cells. As 98% of the material is air, EPS provides good insulating properties
at a low weight. Other characteristics of the material include low moisture absorption, long service life and high compressive
strength.
EPS is manufactured through permeating polystyrene beads with pentane, allowing the beads to expand when exposed to
steam. This addition of a so-called blowing agent adds 4% - 6% w/w. The expanded polystyrene (EPS) beads are then fed into a
block molding machine, where steam and pressure forms large blocks of EPS. The amount of EPS going into the mold
determines the densitiy of the block, where pressure class 80 provides a density at 80 kN/m2, which is approximately 15 kg/m3.
After molding, the remaining blowing agent, pentane, is aired out and the blocks are cut into the desired shape.
Weight per declared unit is approximately 0,57 kg given a density of 15 kg/cubic meter with a thickness of 38 mm.
Technical data
CE marking EPS insulation boards are CE certified according to NS-EN 13163
Typical size 600 mm x 1200 mm
Typical thickness 10 mm - 200 mm
Bending strength >50 kN/m2
Compressive strength 80 kN/m2 (declared unit), see conversion factors for other values
Moisture absorption <5 vol%
Fire class F
Conversion factors
EPS insulation is provided in different densities and thicknesses depending on the intended use. The relationships between
density and weight, and between weight and environmental impacts are linear. Results for various densities and thicknesses
can be converted based on the following factors (factor * environmental impact):
Thickness [mm]
Compressive strength [kN/m2] 38 50 100
60 0.89 1.2 2.3
80 1 1.3 2.6
100 1.2 1.6 3.1
150 1.6 2.1 4.2
200 1.9 2.5 5
250 2.3 3 6
300 2.6 3.4 6.9
400 3.3 4.3 8.7
Product specification
Material use per declared unit kg %
Polystyrene 0.57 94%
Pentane 0.03 6%
Market
Norway
Reference service life, product
60 years
Reference service life, building
60 years
NEPD-2796-1492-EN BEWi EPS 80 EPS Insulation boards (ver1)
3/7
LCA: Calculation rules
Declared unit System boundary
1 m² EPS insulation board with 38 mm thickness at R=1 m² Modules are declared according to NPCR 012 Part B.
K/W, transportation to site, waste handling and recovery. Declared units include A1-A3, A4, C1-C4, and D and are
shown in Figure 1. Gray boxes denote modules not
declared.
System boundary Next system
A1 –A3 Product phase A4 C1 -C4 End-of-life D
Polystyrene Manufacturing Transport to site Deconstruction Energy substitution
• Block molding and beyond system
cutting boundary
Pentane • Packaging of Waste transport
products A5
LPG Wastes Installation on site Waste processing
• Pentane (air)
• Heat (air)
Electricity • Water (water) Disposal
• Solid wastes B1-B7
Packaging/auxiliaries Use phase
Figure 1: System boundaries
Data quality
General requirements and guidelines concerning the use of generic and specific data and the quality of those are as described in
EN 15804: 2012+A1:2013, clause 6.3.6 and 6.3.7., including ISO14044:2006, 4.2.3.6. The data is representative according to
temporal, geographical and technological requirements. Databases used have been ecoinvent v3.6 (2019). Upstream data for
polystyrene from Plastics Europe (2015). Calculations have been carried out using Simapro v9.
Temporal:
Data for use in module A3 is supplied by the EPD owner and consists of recorded and calculated amounts of specific material
and energy consumption. Specific data has been collected for 2019. Generic data has been created or updated within the last 10
years. Any exceptions are documented in the LCA-report.
Geographical:
The product included in this EPD is manufactured in Norway and is representative for the Norwegian market. Best available
proximations are used where Norwegian-specific data are unavailable.
Technological:
Data represents technology in use.
Allocation
The allocation is made in accordance with the provisions of EN 15804. Incoming energy and water and waste production in-
house is allocated equally among all products through mass allocation. Effects of primary production of recycled materials
allocated to the main product in which the material was used. The recycling process and transportation of the material is
allocated to this analysis.
Cut-off criteria
All major raw materials and all the essential energy is included. The production process for raw materials and energy flows that
are included with very small amounts (<1% energy, mass, impact) are not included. This cut-off rule does not apply for hazardous
materials and substances.
Benefits and loads beyond the system boundary (Module D)
The scenario for Module D follows the conservative scenario provided in NPCR 012 Part B. EPS insulation recovered at the end
of life is incinerated with energy recovery and substitutes Norwegian elecitricty and district heat mixes.
NEPD-2796-1492-EN BEWi EPS 80 EPS Insulation boards (ver1)
4/7
LCA: Scenarios and additional technical information
The following information describe the scenarios in the different modules of the EPD.
Transport from production place to user (A4)
Type Type of vehicle Distance km Fuel/Energy Value
Capacity utilisation (incl. return) %
consumption (l/t)
Truck 4.6 % 100 m3 jumbo trailer 300 0.19 l/tkm 57.9
End of Life (C1, C3, C4) Benefits and loads beyond system boundaries (D)
Unit Value Unit Value
Hazardous waste disposed kg Substitution of electricty MJ 1.50
Collected as mixed construction waste kg Substitution of district heating MJ 12.20
Reuse kg
Recycling kg
Energy recovery (C3) kg 0.57
To landfill (C4) kg 0.004
Transport to waste processing (C2)
Type Value
Capacity utilisation (incl. return) %
(l/t)
Truck 4.3% 83 l/tkm
LCA: Results
System boundaries (X=included, MND= module not declared, MNR=module not relevant)
D
lasopsiD
-gnilcyceR-yrevoceR-esueR
laitnetop
C4
X
gnissecorp
etsaW
C2
X
tropsnarT
B7 C1 C3
MND X X X
noitilomed
noitcurtsnoc-eD
A2
X
tropsnarT
esu
ygrene
lanoitarepO
Fuel/Energy
consumption
0.19 15.6
The scenario for transportation to waste processing is assumed to be 83 km (Raadal et al., 2009). Insulation is assumed
compressed at the waste handling facility. A standard box trailer with a 90 m3 cubic capacity is assumed.
Use stage End of life stage
gnirutcafunaM
ylbmessA
esU
ecnanetniaM
riapeR
tnemecalpeR tnemhsibrufeR
esu
retaw
lanoitarepO
Type of vehicle Distance km
Beyond the
system
boundaries
tropsnarT
90 m3 box trailer
Product stage Assemby stage
A1 A3 A4 B1 B2 B5
X X X MND MND MND
slairetam
waR
The scenario for transportation to building site follows the default scenario provided in NPCR 012 Part B. EPS is a bulky
product, resulting in a low capasity utlization (4,6 %).
Due to a lack of reliable data for the removal of EPS insulation from buildings, C1 is assumed to not require energy or
material inputs. The scenario for end-of-life treatment of collected EPS follows the default conservative scenario provided in
NPCR 012 Part B, which is municipal incineration with energy recovery (C3). Ashes and solids after incineration is landfilled
(C4). Recovered energy from C3 is assumed to substitute elecricity and district heating (D).
A5 B3 B4 B6
MND MND MND MND
NEPD-2796-1492-EN BEWi EPS 80 EPS Insulation boards (ver1)
5/7
Environmental impact
Parameter Unit A1-A3 A4 C1 C2 C3 C4 D
GWP kg CO -eqv 2.21E+00 1.12E-01 0.00E+00 3.19E-02 1.81E+00 3.53E-05 -8.94E-03
2
ODP kg CFC11-eqv 1.80E-08 2.54E-08 0.00E+00 7.62E-09 1.25E-09 1.58E-11 -5.68E-10
POCP kg C 2H 4 -eqv 1.42E-02 3.84E-04 0.00E+00 5.26E-05 2.68E-04 3.08E-07 -1.96E-05
AP kg SO 2 -eqv 4.71E-03 3.93E-04 0.00E+00 7.23E-05 2.19E-04 2.77E-07 -3.43E-05
EP kg PO 43--eqv 5.29E-04 2.26E-06 0.00E+00 6.58E-07 1.67E-06 1.95E-07 -3.64E-07
ADPM kg Sb-eqv 4.94E-06 3.36E-07 0.00E+00 9.48E-08 7.47E-08 5.83E-10 -2.14E-07
ADPE MJ 4.87E+01 1.58E+00 0.00E+00 4.75E-01 1.38E-01 1.07E-03 -1.19E-01
GWP Global warming potential; ODP Depletion potential of the stratospheric ozone layer; POCP Formation potential of tropospheric
photochemical oxidants; AP Acidification potential of land and water; EP Eutrophication potential; ADPM Abiotic depletion potential for non
fossil resources; ADPE Abiotic depletion potential for fossil resources
Resource use
Parameter Unit A1-A3 A4 C1 C2 C3 C4 D
RPEE MJ 2.93E+00 6.58E-03 0.00E+00 1.92E-03 4.62E-03 2.49E-05 -1.63E+00
RPEM MJ 0.00E+00 0.00E+00 0.00E+00 0.00E+00 0.00E+00 0.00E+00 0.00E+00
TPE MJ 2.93E+00 6.58E-03 0.00E+00 1.92E-03 4.62E-03 2.49E-05 -1.63E+00
NRPE MJ 2.42E+01 1.58E+00 0.00E+00 4.75E-01 1.38E-01 1.07E-03 -1.19E-01
NRPM MJ 2.45E+01 0.00E+00 0.00E+00 0.00E+00 0.00E+00 0.00E+00 0.00E+00
TRPE MJ 4.87E+01 1.58E+00 0.00E+00 4.75E-01 1.38E-01 1.07E-03 -1.19E-01
SM kg 0.00E+00 0.00E+00 0.00E+00 0.00E+00 0.00E+00 0.00E+00 0.00E+00
RSF MJ 0.00E+00 0.00E+00 0.00E+00 0.00E+00 0.00E+00 0.00E+00 0.00E+00
NRSF MJ 0.00E+00 0.00E+00 0.00E+00 0.00E+00 0.00E+00 0.00E+00 0.00E+00
W
m3
2.46E-02 4.48E-05 0.00E+00 1.29E-05 5.40E-04 1.18E-06 -1.22E-02
RPEE Renewable primary energy resources used as energy carrier; RPEM Renewable primary energy resources used as raw materials;
TPE Total use of renewable primary energy resources; NRPE Non renewable primary energy resources used as energy carrier; NRPM Non
renewable primary energy resources used as materials; TRPE Total use of non renewable primary energy resources; SM Use of secondary
materials; RSF Use of renewable secondary fuels; NRSF Use of non renewable secondary fuels; W Use of net fresh water
End of life - Waste
Parameter Unit A1-A3 A4 C1 C2 C3 C4 D
HW kg 1.06E-03 3.82E-05 0.00E+00 1.13E-05 1.70E-02 2.53E-06 -2.25E-05
NHW kg 1.15E-01 2.16E-02 0.00E+00 6.01E-03 9.56E-03 3.68E-03 -9.37E-03
RW kg 9.29E-06 1.13E-05 0.00E+00 3.39E-06 3.11E-07 7.16E-09 -1.11E-06
HW Hazardous waste disposed; NHW Non hazardous waste disposed; RW Radioactive waste disposed
End of life - Output flow
Parameter Unit A1-A3 A4 C1 C2 C3 C4 D
CR kg 0.00E+00 0.00E+00 0.00E+00 0.00E+00 0.00E+00 0.00E+00 0.00E+00
MR kg 0.00E+00 0.00E+00 0.00E+00 0.00E+00 0.00E+00 0.00E+00 0.00E+00
MER kg 1.19E-02 0.00E+00 0.00E+00 0.00E+00 5.70E-01 0.00E+00 0.00E+00
EEE MJ 0.00E+00 0.00E+00 0.00E+00 0.00E+00 1.50E+00 0.00E+00 0.00E+00
ETE MJ 0.00E+00 0.00E+00 0.00E+00 0.00E+00 1.22E+01 0.00E+00 0.00E+00
CR Components for reuse; MR Materials for recycling; MER Materials for energy recovery; EEE Exported electric energy; ETE Exported
thermal energy
Reading example: 9,0 E-03 = 9,0*10-3 = 0,009
NEPD-2796-1492-EN BEWi EPS 80 EPS Insulation boards (ver1)
6/7
Additional Norwegian requirements
Greenhous gas emission from the use of electricity in the manufacturing phase
Norwegian production mix from import, medium voltage (production of transmission lines, in addition to direct emissions and
losses in grid) of applied electricity for the manufacturing prosess(A3).
Data source Amount Unit
Econinvent v3.6 0.022 kg CO -eqv/kWh
2
Dangerous substances
The product contains no substances given by the REACH Candidate list or the Norwegian priority list
The product contains substances given by the REACH Candidate list or the Norwegian priority list that are less than 0,1 %
by weight.
The product contain dangerous substances, more then 0,1% by weight, given by the REACH Candidate List or the
Norwegian Priority list, see table.
The product contains no substances given by the REACH Candidate list or the Norwegian priority list. The product is
classified as hazardous waste (Avfallsforskiften, Annex III), see table.
Indoor environment
No tests have been carried out on the product concerning indoor climate - Not relevant.
Carbon footprint
Carbon footprint has not been worked out for the product.
Bibliography
ISO 14025:2010 Environmental labels and declarations - Type III environmental declarations - Principles
and procedures
ISO 14044:2006 Environmental management - Life cycle assessment - Requirements and guidelines
EN 15804:2012+A1:2013 Sustainability of construction works - Environmental product declaration - Core rules for
the product category of construction products
ISO 21930:2007 Sustainability in building construction - Environmental declaration of building products
Jennssen, M.M. (2020) LCA report: EPS insulation, for BEWI ASA
NPCR 012:2018 Part B for Thermal insulation products
Raadal et al. (2009) Klimaregnskap for avfallshåndtering. Fase I og II: Glassemballasje, metallemballasje,
papir, papp, plastemballasje, våtorganisk avfall, treavfall og restavfall fra husholdninger.
ISBN: 82-8035-073-X.
Publisher/Program operator Phone: +47 23 08 80 00
The Norwegian EPD Foundation
Post Box 5250 Majorstuen, 0303 Oslo e-mail: post@epd-norge.no
Norway web epd-norge.no
Owner of the declaration Phone: +47 72 44 88 88
BEWI ASA Fax
Hamarvikringen 64, 7263 Hamarvik e-mail: ordre@bewi.com
Norway web bewi.com
Author of the Life Cycle Assessment Phone: +47 41 79 94 17
Michael M. Jenssen Fax
Asplan Viak AS e-mail: asplanviak@asplanviak.no
Abels gate 9, 7030 Trondheim, Norway web asplanviak.no
NEPD-2796-1492-EN BEWi EPS 80 EPS Insulation boards (ver1)
7/7
