ENVIRONMENTAL PRODUCT DECLARATION
as per ISO 14025 and EN 15804+A2
Owner of the Declaration Knauf Ceiling Solutions GmbH & Co. KG
Publisher Institut Bauen und Umwelt e.V. (IBU)
Programme holder Institut Bauen und Umwelt e.V. (IBU)
Declaration number EPD-KNA-20240023-IBI1-EN
Issue date 12.03.2024
Valid to 11.03.2029
Bioguard Plain, ANF
Knauf Ceiling Solutions GmbH & Co. KG
www.ibu-epd.com | https://epd-online.com
1. General Information
Knauf Ceiling Solutions GmbH & Co. KG Bioguard Plain, ANF
Programme holder Owner of the declaration
IBU – Institut Bauen und Umwelt e.V. Knauf Ceiling Solutions GmbH & Co. KG
Hegelplatz 1 Elsenthal 15
10117 Berlin 94481 Grafenau
Germany Germany
Declaration number Declared product / declared unit
EPD-KNA-20240023-IBI1-EN 1 m² Bioguard Plain mineral ceiling tiles with a surface weight of
3.29 kg/m², also representative for 1 m² of ANF mineral ceiling tiles with a
surface weight of 2.92 kg/m²
This declaration is based on the product category rules: Scope:
Mineral panels, 01.08.2021 This document refers to 1 m² Bioguard Plain ceiling tiles with a surface
(PCR checked and approved by the SVR) weight of 3.29 kg/m², manufactured at the production facility in Wujiang,
China.
Results for Bioguard Plain are also representative for 1 m² of ANF mineral
Issue date ceiling tiles with a surface weight of 2.92 kg/m², manufactured at the
production facility in Wujiang, China (when deducting 10 % of the
12.03.2024
environmental impact of the results of Bioguard Plain).
The owner of the declaration shall be liable for the underlying information
Valid to
and evidence; the IBU shall not be liable with respect to manufacturer
11.03.2029 information, life cycle assessment data and evidences.
The EPD was created according to the specifications of EN 15804+A2. In
the following, the standard will be simplified as EN 15804.
Verification
The standard EN 15804 serves as the core PCR
Independent verification of the declaration and data according to ISO
14025:2011
internally X externally
Dipl.-Ing. Hans Peters
(Chairman of Institut Bauen und Umwelt e.V.)
Florian Pronold Vito D'Incognito,
(Managing Director Institut Bauen und Umwelt e.V.) (Independent verifier)
1 Environmental Product Declaration - Knauf Ceiling Solutions GmbH & Co. KG - Bioguard Plain, ANF
2. Product
substances listed in the ECHA-candidate list (date: 25.06.2020)
2.1 Product description/Product definition exceeding 0.1 percentage by mass: No.
The ceiling tiles are manufactured using a wet-felt process and
consist of biosoluble mineral wool, perlite, clay and starch. In This product/article/at least one partial article contains other
addition, the visible side of the mineral tile is painted with carcinogenic, mutagenic, reprotoxic (CMR) substances in
dispersion paint. The back side is primed with dispersion paint. categories 1A or 1B which are not on the candidate list,
exceeding 0.1 percentage by mass: No.
The mineral tiles are available in different formats and edge
finishes. Biocide products were added to this construction product or it
has been treated with biocide products (this then concerns a
This EPD applies to the following products: treated product as defined by the (EU) Ordinance on Biocide
Products No. 528/2012): No.
Bioguard Plain
ANF In-can preservatives are used in the production process;
however, they are not part of the products and are therefore not
For the use and application of the product, the respective within the scope of the Ordinance on Biocide Products.
national provisions at the place of use apply, in Germany for
example the building codes of the federal states and the 2.6 Manufacture
corresponding national specifications. The mineral tiles are produced in the traditional wet process
(wet-felt). The raw materials are mixed with water to form a
2.2 Application homogeneous suspension, which is pumped onto a belt
Mineral tiles (wet-felt) are typically used as lay-in for suspended conveyor (Fourdrinier). The water is removed mechanically
ceiling constructions. They are primarily used as optical (gravity and vacuum) and by evaporation in the drying oven. As
cladding, but also for sound absorption and sound insulation, far as possible, the process water is reused. It is treated
for fire resistance and against fire spreading, for cleanrooms accordingly and fed back into the process water circuit.
and high hygiene requirements. Production waste and dust are reused in the process in the
sense of an internal cycle. The manufacturing plant is certified
2.3 Technical Data
according to ISO 9001, ISO 14001 and ISO 45001.
2.7 Environment and health during manufacturing
Construction data
Name Value Unit • The manufacturing plant is certified according to ISO
9001, ISO 14001 and ISO 45001.
0.05 -
Thermal conductivity W/(mK) • The production has a closed water cycle.
0.06
• Production generates almost no waste, resulting blanks,
Fire Test on Building Materials and
Class 1 dust and rejects are reused.
Structures acc. BS 476 part 7
• Not subject to declaration according to REACH.
Fire Propagation Index acc. BS 476 part 6 10.28
Formaldehyde after 52 h < 0.005 mg/m³ 2.8 Product processing/Installation
TVOC after 72 h 0.064 mg/(m²*h) There are no recognised systemic hazards associated with the
installation of ceiling tiles. It is recommended that materials are
handled in a manner that minimises dust generation. Workers
Performance data of the product with respect to its
should wear appropriate personal protective equipment.
characteristics in accordance with the relevant technical
Equipment such as gloves, goggles and dust masks are
provision (no CE-marking).
recommended to minimise exposure to dust and prevent skin
irritation.
2.4 Delivery status
The EPD refers to panels with a thickness of 16 mm which can 2.9 Packaging
have variable length and width dimensions.
The panels are packaged in cardboard boxes and sealed with
transparent polyethylene film. These packages lie on
2.5 Base materials/Ancillary materials
chemically untreated wooden pallets. The pallets are wrapped
Mineral tile composition: with polyethylene stretch film. Foil, paper and wood can be
Name Value Unit recycled in the usual ways.
Mineral wool 10 %
2.10 Condition of use
Perlite 40-42 %
When handled properly, the mechanical and structural-physical
Clay 5 % properties of the mineral tile remain intact throughout its entire
Paper 10-12 % service life. Direct contact with water should be avoided due to
Starch 5 % the water-soluble binding agent starch.
Brokes/dust (internally looped production waste) 26 % 2.11 Environment and health during use
When properly installed, no dust/particles are released during
In addition, the visible side of the mineral tile is painted with the use phase. For the substance groups formaldehyde, volatile
dispersion paint. The back side is primed with a dispersion organic compounds (VOCs) and total volatile organic
paint. compounds (TVOCs), the limits according to GB/T 17657-2013
The recycled content is not less than 20-22 %. and HJ 571-2010 are complied with.
This product/article/at least one partial article contains
2 Environmental Product Declaration - Knauf Ceiling Solutions GmbH & Co. KG - Bioguard Plain, ANF
2.12 Reference service life Mechanical destruction
The service life of the mineral tiles (wet-felted) is up to The mineral slabs (wet-felt) can be broken by hand and also
50 years, depending on the area of use, exposure and state of damaged superficially, which can result in minor dust formation.
maintenance. Within the framework of the conditions of use, no
ageing effects are to be expected apart from visual 2.14 Re-use phase
discolouration caused by air circulation. If the panels are removed properly, they can be reinstalled. In
case of minor damage, the slabs can be reused as cut-to-size
2.13 Extraordinary effects tiles. Mineral tiles can be returned to the manufacturing process
Fire if they are of the correct type and have sufficient material
The declared products are classified in the fire reaction class 1 quality; they can be recycled up to 100 %.
according to BS 476 Part 6.
2.15 Disposal
Water The waste code number of production residues for mineral tiles
In the case of prolonged contact with water, the starch binder according to the AVV, German List of Wastes Ordinance is 10
dissolves, which can lead to a loss of structure, and if the 11 03, the waste code number for construction site waste
soluble components are discharged into the sewage treatment (offcuts) is 17 06 04. If the tiles are not recycled as described in
plant, they are biodegradable, increasing the chemical oxygen 2.14., they are disposed of in a landfill.
demand (COD) and biological oxygen demand (BOD).
2.16 Further information
Further information at www.knaufceilingsolutions.com
3. LCA: Calculation rules
3.1 Declared Unit Module C3 | Waste processing
This EPD refers to a declared unit of 1 m² Bioguard Plain The declared scenario assumes landfilling of the product.
mineral ceiling tiles with a surface weight of 3.29 kg/m². Referring environmental impacts are accounted for in module
Declared Unit C4.
Name Value Unit
Module C4 | Disposal
Declared unit 1 m2 Module C4 refers to the emissions from the disposal of the
Grammage (with coating) 3.29 kg/m2 mineral ceiling tiles. The chosen scenario, therefore, includes
Layer thickness 0.016 m the environmental burdens of landfilling the product.
Boardmill density (raw board, without coating) 200 kg/m³
Module D | Benefits and loads beyond the system
boundary
The ceiling tiles are produced at the Knauf Ceiling Solutions The declared scenario assumes landfilling of the product.
production site in Wujiang, China. Referring environmental impacts are accounted for in module
Various types of mineral ceiling tiles are produced at the site. C4.
Product-specific results for 1 m² of ANF mineral ceiling tiles with
a surface weight of 2.92 kg/m² can be approximated deducting 3.3 Estimates and assumptions
10 % of the environmental impact of the results of Bioguard Assumptions and approximations are applied in case of a lack
Plain. of representative data. All assumptions and approximations are
documented precisely and represent a best-guess
3.2 System boundary representation of reality. In case of uncertainty, a conservative
The life cycle assessment of Bioguard Plain mineral ceiling tiles approach is chosen.
includes a cradle-to-gate analysis of the products'
environmental impacts with modules (A1–A3, C, D). This study builds on Chinese background data as far as
Subsequent life cycle phases are part of the analysis: supported by the available databases. Nevertheless, some
upstream supply chains of used raw materials were
Module A1–A3 | Production stage approximated via European data, due to a lack of
The production stage includes the upstream burdens of raw geographically adapted datasets.
material supply, their transports and the manufacturing plant of
Knauf Ceiling Solutions located in Wujiang (China). Mineral 3.4 Cut-off criteria
ceiling tiles are produced in the wet-felt process. Main raw The LCA model covers all available input and output flows,
material inputs, therefore, refer to mineral wool, perlite, clay and which can be represented based on robust data. Data gaps are
starch. The production site is supplied with electricity from the filled with conservative assumptions from average data (when
Chinese power grid and thermal energy from natural gas. available) or with generic data and are documented
accordingly. Only data with a contribution lower than 1 % were
Module C1 | Deconstruction and demolition cut off. Thus, no data were neglected, of which a substantial
Disassembly of the product is done either manually or using impact is to be expected. All relevant data were collected
smaller tools. Referring energy demand is considered to be comprehensively. Cut-off material and energy flows were
negligible. chosen carefully based on their expected quantitative
contribution as well as potential environmental impacts. Thus, it
Modul C2 | Transport to disposal can be assumed that the sum of all neglected input flows does
The transport to the disposal of the material is estimated not account for more than 5 % of the total material, water and
declaring a 50 km radius to the landfill. In reality, this scenario energy flows.
may vary depending on the actual location of deconstruction
and referring waste treatment.
3 Environmental Product Declaration - Knauf Ceiling Solutions GmbH & Co. KG - Bioguard Plain, ANF
3.5 Background data 3.8 Geographic Representativeness
This study uses generic background data for the evaluation of Land or region, in which the declared product system is
upstream environmental impacts from GaBi databases (GaBi manufactured, used or handled at the end of the product´s
10; 2022.2). lifespan: China
3.6 Data quality
Data collection is based on product-specific questionnaires. It 3.9 Allocation
follows an iterative process of clarifying questions via e-mail, All information for the allocation of given material and energy
telephone calls or in personal/web meetings. Intensive flows is based on site-related evaluations. The calculation of
discussions between Knauf Ceiling Solutions and Daxner & specific input quantities for the raw board production is based
Merl result in an accurate mapping of product-related material on the respective recipe. In addition, product-specific
and energy flows. This leads to a high quality of foreground application rates (e.g. backcoat, primer etc.) were available.
data collected. Data collection relies on a consistent process Total annual energy consumption and waste flows are allocated
according to ISO 14044. based on the production share of the product.
The technological, geographical and time-related For in the production used waste paper, the system boundary is
representativeness of the database was kept in mind when set after sorting. It is assumed that the end-of-waste status has
selecting background data. Whenever specific data were been reached. The system boundary for secondary raw
missing, either generic datasets or representative average data materials defined in EN 15804 applies.
were used instead. The implemented GaBi background
3.10 Comparability
datasets refer to the latest versions available (not more than
ten years old) and are carefully chosen. Basically, a comparison or an evaluation of EPD data is only
possible if all the data sets to be compared were created
3.7 Period under review according to EN 15804 and the building context, respectively
Foreground data were collected in the 2021 production year, the product-specific characteristics of performance, are taken
and the data are based on the volumes produced on an annual into account.
basis.
The GaBi background database was used to calculate the LCA
(GaBi 10; 2022.2).
4. LCA: Scenarios and additional technical information
Characteristic product properties of biogenic carbon
The biogenic carbon content quantifies the amount of biogenic
carbon in the declared product.
Installation in building (A5)
Information on the description of the biogenic carbon The End-of-Life of the product packaging materials is not
content at the factory gate declared in module A5.
Name ValueUnit Name Value Unit
Biogenic carbon content in product 0.28 kg Packaging (cardboard) 0.009 kg/m²
C
Packaging (PE-film) 0.035 kg/m²
Biogenic carbon content in accompanying kg
0.015
packaging C
End-of-Life (C1–C4)
Note: 1 kg of biogenic carbon is equivalent to 44/12 kg of CO .
2
Name Value Unit
The carbon stored in the packaging was taken into account as Collected separately 3.29 kg
"CO 2-neutral". Thus the storage effect of the carbon bound in Landfilling 3.29 kg
the packaging is not included in the calculation but is
considered as emitted immediately.
4 Environmental Product Declaration - Knauf Ceiling Solutions GmbH & Co. KG - Bioguard Plain, ANF
5. LCA: Results
The following table contains the LCA results for a declared unit of 1 m² Bioguard Plain mineral ceiling tiles with a surface weight of
3.29 kg/m².
DESCRIPTION OF THE SYSTEM BOUNDARY (X = INCLUDED IN LCA; MND = MODULE OR INDICATOR NOT DECLARED; MNR
= MODULE NOT RELEVANT)
Benefits and
Construction loads beyond
Product stage Use stage End of life stage
process stage the system
boundaries
la ire ta m w a Ry lp p u s tro p s n a rT g n iru tc a fu n a M e h t m o rf tro p s n a rTe tis e h t o t e ta g y lb m e s s A e s U e c n a n e tn ia M ria p e R tn e m e c a lp e R tn e m h s ib ru fe R y g re n e la n o ita re p Oe s u re ta w la n o ita re p Oe s u n o itc u rts n o c -e Dn o itilo m e d tro p s n a rT g n is s e c o rp e ts a W la s o p s iD -e s u e R-y re v o c e R-g n ilc y c e Rla itn e to p
A1 A2 A3 A4 A5 B1 B2 B3 B4 B5 B6 B7 C1 C2 C3 C4 D
X X X MND MND MND MND MNR MNR MNR MND MND X X X X X
RESULTS OF THE LCA - ENVIRONMENTAL IMPACT according to EN 15804+A2: 1 m² Bioguard Plain ceiling tiles (3.29 kg/m²)
Parameter Unit A1-A3 C1 C2 C3 C4 D
Global Warming Potential total (GWP-total) kg CO 2 eq 1.58E+01 0 1.03E-02 0 1.09E+00 0
Global Warming Potential fossil fuels (GWP-fossil) kg CO 2 eq 1.69E+01 0 9.87E-03 0 4.91E-02 0
Global Warming Potential biogenic (GWP-biogenic) kg CO 2 eq -1.02E+00 0 4.37E-04 0 1.04E+00 0
Global Warming Potential luluc (GWP-luluc) kg CO 2 eq 1.18E-02 0 2.57E-07 0 9.06E-05 0
Depletion potential of the stratospheric ozone layer (ODP) kg CFC11 eq 1.98E-10 0 9.68E-16 0 1.15E-13 0
Acidification potential of land and water (AP) mol H+ eq 5.09E-02 0 3.31E-05 0 3.48E-04 0
Eutrophication potential aquatic freshwater (EP-freshwater) kg P eq 7.27E-05 0 1.25E-09 0 8.32E-08 0
Eutrophication potential aquatic marine (EP-marine) kg N eq 1.24E-02 0 1.5E-05 0 8.9E-05 0
Eutrophication potential terrestrial (EP-terrestrial) mol N eq 1.31E-01 0 1.65E-04 0 9.78E-04 0
Formation potential of tropospheric ozone photochemical oxidants kg NMVOC
3.81E-02 0 2.99E-05 0 2.7E-04 0
(POCP) eq
Abiotic depletion potential for non fossil resources (ADPE) kg Sb eq 2.45E-04 0 4E-10 0 5.03E-09 0
Abiotic depletion potential for fossil resources (ADPF) MJ 2.61E+02 0 1.36E-01 0 6.43E-01 0
m3 world eq
Water use (WDP) 4.95E+00 0 8.4E-05 0 5.38E-03 0
deprived
RESULTS OF THE LCA - INDICATORS TO DESCRIBE RESOURCE USE according to EN 15804+A2: 1 m² Bioguard Plain ceiling
tiles (3.29 kg/m²)
Parameter Unit A1-A3 C1 C2 C3 C4 D
Renewable primary energy as energy carrier (PERE) MJ 9.57E+01 0 7.39E-04 0 9.65E-02 0
Renewable primary energy resources as material utilization
MJ 1.2E+01 0 0 0 0 0
(PERM)
Total use of renewable primary energy resources (PERT) MJ 1.08E+02 0 7.39E-04 0 9.65E-02 0
Non renewable primary energy as energy carrier (PENRE) MJ 2.6E+02 0 1.37E-01 0 6.44E-01 0
Non renewable primary energy as material utilization (PENRM) MJ 3.91E-01 0 0 0 0 0
Total use of non renewable primary energy resources (PENRT) MJ 2.61E+02 0 1.37E-01 0 6.44E-01 0
Use of secondary material (SM) kg 1.36E-01 0 0 0 0 0
Use of renewable secondary fuels (RSF) MJ 0 0 0 0 0 0
Use of non renewable secondary fuels (NRSF) MJ 0 0 0 0 0 0
Use of net fresh water (FW) m3 1.64E-01 0 2.12E-06 0 1.63E-04 0
RESULTS OF THE LCA – WASTE CATEGORIES AND OUTPUT FLOWS according to EN 15804+A2:
1 m² Bioguard Plain ceiling tiles (3.29 kg/m²)
Parameter Unit A1-A3 C1 C2 C3 C4 D
Hazardous waste disposed (HWD) kg 3.14E-06 0 3.42E-13 0 3.31E-11 0
Non hazardous waste disposed (NHWD) kg 2.99E+00 0 5.66E-06 0 3.29E+00 0
Radioactive waste disposed (RWD) kg 1.04E-02 0 7.69E-08 0 7.15E-06 0
Components for re-use (CRU) kg 0 0 0 0 0 0
Materials for recycling (MFR) kg 0 0 0 0 0 0
Materials for energy recovery (MER) kg 0 0 0 0 0 0
Exported electrical energy (EEE) MJ 0 0 0 0 0 0
Exported thermal energy (EET) MJ 0 0 0 0 0 0
RESULTS OF THE LCA – additional impact categories according to EN 15804+A2-optional:
1 m² Bioguard Plain ceiling tiles (3.29 kg/m²)
Parameter Unit A1-A3 C1 C2 C3 C4 D
Incidence of disease due to PM emissions (PM) Disease 5.32E-07 0 1.78E-10 0 4.28E-09 0
5 Environmental Product Declaration - Knauf Ceiling Solutions GmbH & Co. KG - Bioguard Plain, ANF
incidence
Human exposure efficiency relative to U235 (IR) kBq U235 eq 1.7E+00 0 5.1E-06 0 7.94E-04 0
Comparative toxic unit for ecosystems (ETP-fw) CTUe 8.29E+01 0 1.62E-01 0 3.6E-01 0
Comparative toxic unit for humans (carcinogenic) (HTP-c) CTUh 6.6E-08 0 2.59E-12 0 5.5E-11 0
Comparative toxic unit for humans (noncarcinogenic) (HTP-nc) CTUh 7.51E-06 0 8.99E-11 0 6.09E-09 0
Soil quality index (SQP) SQP 4.15E+02 0 4.03E-04 0 1.34E-01 0
Disclaimer 1 – for the indicator 'Potential Human exposure efficiency relative to U235'.
This impact category deals mainly with the eventual impact of low-dose ionizing radiation on human health of the nuclear fuel cycle. It
does not consider effects due to possible nuclear accidents, occupational exposure or radioactive waste disposal in underground
facilities. Potential ionizing radiation from the soil, radon and from some construction materials is also not measured by this indicator.
Disclaimer 2 – for the indicators 'abiotic depletion potential for non-fossil resources', 'abiotic depletion potential for fossil resources',
'water (user) deprivation potential, deprivation-weighted water consumption', 'potential comparative toxic unit for ecosystems', 'potential
comparative toxic unit for humans – cancerogenic', 'Potential comparative toxic unit for humans - not cancerogenic', 'potential soil
quality index'.
The results of this environmental impact indicator shall be used with care as the uncertainties on these results are high as there is
limited experience with the indicator.
6. LCA: Interpretation
The following interpretation contains a summary of the LCA mineral ceiling tiles.
results referenced to a declared unit of 1 m² Bioguard Plain
The comparison of the product's life cycle phases shows a The upstream supply chain of the raw board plays a dominant
clear dominance of the production phase (modules A1–A3) in role in all categories.
all environmental impact categories. The potential
environmental impacts from transport to disposal (module C2) Based on the results of Bioguard Plain, the environmental
and the End of Life of the products due to landfilling (module impact of ANF is overestimated by about 10 % in all
C4) have a minor contribution. environmental impact categories.
7. Requisite evidence
7.1 Radioactivity Measuring point: Fraunhofer Institute for Toxicology and
Not applicable for these products. Experimental Medicine
Certificate number: 02G15015 (5 September 2016)
7.2 Biopersistence Test substance: Slag Wool 'Arm SW15'
The mineral wool used for the production of the panels is
biosoluble.
6 Environmental Product Declaration - Knauf Ceiling Solutions GmbH & Co. KG - Bioguard Plain, ANF
7.3 VOC emissions
Test results
Measuring point: China National Fiberglass Product Quality
Name Value Unit
Inspection & Testing Center
Test report: VOC emissions test report TVOC after 72h 0.064 mg/(m²*h)
Report No: 23102128 Formaldehyde after 52h <0.005 mg/m³
Testing periode: 8.10.2023-8.11.2023
Test basis: GB/T 25998-2020 & HJ 571-2010
8. References
Standards (Federal Law Gazette I p. 3005).
ASTM C423-01 Chemicals Prohibition Ordinance
ASTM C423-01:2001-07, Standard Test Method for Sound Chemicals Prohibition Ordinance (German designation:
Absorption and Sound Absorption Coefficients by the Chemikalien-Verbotsverordnung – ChemVerbotsV) of 20
Reverberation Room Method. January 2017 (Federal Law Gazette I p. 94; 2018 I p. 1389),
last amended by Article 300 of the Ordinance of 19 June 2020
ASTM E413-10 (Federal Law Gazette I p. 1328).
ASTM E413-10:2010-09, Classification for Rating Sound
Insulation. China National Fiberglass Product Quality Inspection &
Testing Center
BS 476 Part 6 Test report: VOC emission test
BS 476 part 6:1989+A1:2009, Fire tests on building materials Report No: 23102128
and structures. Method of test to determine the classification of
the surface spread of flame of products. ECHA-candidate list
List of substances of very high concern (SVHC) for
DIN 18177 authorisation (ECHA Candidate List), 25.06.2020, published
DIN 18177:2020-12, Wet-felt factory-produced mineral panels. under Article 59(10) of REACH. Helsinki: European Chemicals
Agency.
GB/T 25998
GB/T 25998, Mineral wool decorating and acoustic ceilings. Fraunhofer Institute for Toxicology and Experimental
Medicine
HJ 571-2010 Certificate number: 02G15015 (5 September 2016); Test
HJ 571-2010, Technical requirement for environmental labelling substance: Slag Wool 'Arm SW15'.
products – Wood-based panels and finishing products.
GaBi
EN 15804 GaBi 10, Software-System and Database for Life Cycle
DIN EN 15804:2012+A2:2019+AC:2021, Sustainability of Engineering. DB 2022.2. Sphera, 1992–2022. Available at:
construction works – Environmental product declarations – https://gabi.sphera.com/support/gabi/
Core rules for the product category of construction products.
IBU 2021
ISO 9001 Institut Bauen und Umwelt e.V.: General instructions for the
DIN EN ISO 9001:2015-11, Quality management systems – EPD programme of Institut Bauen und Umwelt e.V. (IBU).
Requirements. Version 2.0, Berlin: Institut Bauen und Umwelt e.V., 2021.
www.ibuepd.com
ISO 14001
DIN EN ISO 14001:2015-11, Environmental management Ordinance on Biocide Products
systems – Requirements with guidance for use. Regulation (EU) No 528/2012 of the European Parliament and
of the Council of 22 May 2012 concerning the making available
ISO 14025 on the market and use of biocidal products.
DIN EN ISO 14025:2011-10, Environmental labels and
declarations – Type III environmental declarations – Principles Ordinance on Hazardous Substances
and procedures. Ordinance on Hazardous Substances, of 26 November 2010
(Federal Law Gazette I p. 1643, 1644), last amended by Article
ISO 14044 148 of the Law of 29 March 2017 (Federal Law Gazette I p.
DIN EN ISO 14044:2006-10, Environmental management – Life 626).
cycle assessment – Requirements and guidelines.
PCR Part A
ISO 45001 Product category rules for building-related products and
DIN ISO 45001:2018-06, Occupational health and safety services. Part A: Calculation rules for the life cycle assessment
management systems – Requirements with guidance for use. and requirements on the project report according to
EN15804+A2:2019. Version 1.3, Berlin: Institut Bauen und
Umwelt e.V. (Hrsg.), 2022.
Further References
PCR: Mineral panels
AVV, German List of Wastes Ordinance Institut Bauen und Umwelt e.V. (IBU), 2023. Product Category
Regulation on the European Waste List. Waste Catalogue Rules for Building-Related Products and Services. Part B:
Ordinance (German designation: Abfallverzeichnisverordnung – Requirements on the EPD for Mineral panels. Version v2,
AVV) of 10 December 2001 (Federal Law Gazette I p. 3379), 31.05.2023.
last amended by Article 1 of the Ordinance of 30 June 2020
7 Environmental Product Declaration - Knauf Ceiling Solutions GmbH & Co. KG - Bioguard Plain, ANF
REACH Registration, Evaluation, Authorisation and Restriction of
Regulation (EC) No 1907/2006 of the European Parliament and Chemicals (REACH).
Council from 18 December 2006, Regulation concerning the
8 Environmental Product Declaration - Knauf Ceiling Solutions GmbH & Co. KG - Bioguard Plain, ANF
Publisher
Institut Bauen und Umwelt e.V. +49 (0)30 3087748- 0
Hegelplatz 1 info@ibu-epd.com
10117 Berlin www.ibu-epd.com
Germany
Programme holder
Institut Bauen und Umwelt e.V. +49 (0)30 3087748- 0
Hegelplatz 1 info@ibu-epd.com
10117 Berlin www.ibu-epd.com
Germany
Author of the Life Cycle Assessment
Daxner & Merl GmbH +43 676 849477826
Lindengasse 39/8 office@daxner-merl.com
1070 Wien www.daxner-merl.com
Austria
Owner of the Declaration
Knauf Ceiling Solutions GmbH & Co. KG 0049 8552 422 0
Elsenthal 15 info@knaufamf.com
94481 Grafenau www.knaufceilingsolutions.com
Germany
9 Environmental Product Declaration - Knauf Ceiling Solutions GmbH & Co. KG - Bioguard Plain, ANF
