Environmental Product
Declaration
as per ISO 14025 and EN 15804+A2
Owner of the declaration: BOSTIK AB
Publisher: Kiwa-Ecobility Experts
Programme operator: Kiwa-Ecobility Experts
Registration number: EPD-Kiwa-EE-000370-EN
Issue date: 08.09.2022
Valid to: 08.09.2027
Bostik Tätskiktsfolie Pro LX
Waterproofing membrane to be applied under ceramic tiles and natural stones
1. General information
BOSTIK AB Bostik Tätskiktsfolie Pro LX
Programme operator Owner of the declaration
Kiwa-Ecobility Experts BOSTIK AB
Voltastr. 5 Strandbadsvägen 22
13355 Berlin 251 09 Helsingborg
Germany Sweden
Registration number Declared product / declared unit
EPD-Kiwa-EE-000370-EN 1 m2 of waterproofing membrane
This declaration is based on the Product Scope
Category Rules Tätskiktsfolie Pro LX is a waterproofing mem-
PCR B - Plastic and rubber sheets for roof, wall, brane to be applied under ceramic tiles and
and floor waterproofing, 2021-12-28 (draft) natural stones. The EPD refers to the specific
Issue date product.
08.09.2022 EPD type: Cradle to gate with options, and
with modules C1-C4 and module D
Valid to Kiwa-Ecobility Experts shall not be liable with
08.09.2027 respect to manufacturer information, life cy-
cle assessment data and evidence.
Verification
The European standard EN 15804+A2:2019
serves as the core PCR.
Independent verification of the declaration
and data according to ISO 14025:2006
☐internal ☒external
Frank Huppertz
(Head of Kiwa-Ecobility Experts)
Prof. Dr. Frank Heimbecher Max Sonnen – Ecomatters
(Chairman of the independent expert committee – Kiwa- (Third party verifier)
Ecobility Experts)
Page | 2 BOSTIK AB – Tätskiktsfolie Pro LX
2. Product
2.1 Product description
Tätskiktsfolie Pro LX is a 3-ply waterproofing membrane made of polyethylene (PE) membrane and
two outer layers of polypropylene (PP) non-woven.
2.2 Application
The sealing membrane should be applied under ceramic tiles and natural stones for perfect water-
proofing. The product is suitable for example for the following typical areas: domestic bathrooms,
commercial kitchens, public and domestic shower rooms, and wet areas.
2.3 Technical data
Essential characteristics Unit Performance
Resistance to temperature: min./max. °C - 30°C / + 90°C
Physical properties
Total Weight (internal) gm/m2 200 (+/- 20)
Length per Roll (internal) m/% 30 (0,0m / + 1%)
Breaking load longitudinal (DIN EN ISO 527-3) N/mm 270/50 (≥ 200 / 50)
Breaking load lateral (DIN EN ISO 527-3) N/mm 170/50 (≥ 100 / 50)
Extension break longitudinal (DIN EN ISO 527-3) % 60 (≥ 30)
Extension break lateral (DIN EN ISO 527-3) % 70 (≥ 40)
Resistance to tearing longitudinal (DIN EN 12310-2) N 100 (≥ 70)
Resistance to tearing lateral (DIN EN 12310-2) N 65 (≥ 25)
Resistance to water pressure (DIN EN 1928 Version B) bar ≥ 1.5
UV-Resistance (DIN EN ISO 4892-3) h ≥ 450
Moisture vapour resistance air equivalent (sd) (DIN EN 1931) m ≥ 75
Bonding strength (DIN EN 1348) N/mm2 ≥ 0.5 (≥ 0.2)
Burst Pressure (Internal) bar ≥ 2.0
Fire Classification (DIN EN 4102 EN 13501-1) - B2
2.4 Placing on the market/ Application rules
The product has received the ETA 022 for Watertight covering kits for wet room floors and or walls.
For the product use the respective national provisions shall apply. In Germany, the product is regulated
in accordance with DIN 18534 for waterproofing for indoor applications. The products are packed and
transported as rolls, and mainly distributed at the European market.
2.5 Base materials / Ancillary materials
Tätskiktsfolie Pro LX contains PP non-woven, LDPE sealing layer, PE colour batch, printing ink and sol-
vent.
Raw material Unit Value
Polypropylene (PP) non-woven % 36-44
Low-density polyethylene (LDPE) sealing layer % 54-62
Colour batch polyethylene (PE) % 1.5-3.5
Printing Ink and solvent % 0.4-1.5
There is no biogenic carbon in the product.
Substances from the “Candidate list of substances of very high concern for authorisation” (SVHC) that
the product contains are according to REACH lower then 0.1%.
Page | 3 BOSTIK AB – Tätskiktsfolie Pro LX
2.6 Manufacturing
The manufacturing is located in Germany [production site code: 001]. The top and bottom non-woven
(PP) are already supplied and delivered as a finished product. The non-wovens are laminated to the up
and downside during extrusion process of the LDPE sealing layer. Subsequently a logo is printed on the
product, and it is cut in size. Finally, the rolls are stacked on reusable pallets and in packed in foil.
The manufacturing process is shown in figure 1.
2.7 Packaging
The waterproofing membranes are wrapped on a cardboard winding tube. The rolls are than packed
in PE film and stacked on reusable pallets, which are also packed in PE plastic film. All packaging mate-
rials are recyclable or reusable (pallets).
2.8 Reference Service Life (RSL)
The Tätskiktsfolie Pro LX sealing membrane has been tested according to EAD 030436-00-0503 (ETAG
022). Receipt of an EAD confirms a RSL of 25 years.
2.9 Other Information
For further information please visit the official webpage under the following link https://www.bos-
tik.com/sweden/sv/catalog/product/construction/emea/sweden/product-t-tskiktsfolie-pro-lx/
Page | 4 BOSTIK AB – Tätskiktsfolie Pro LX
Figure 1: Process flow chart of the production of Tätskiktsfolie Pro LX
Page | 5 BOSTIK AB – Tätskiktsfolie Pro LX
3. LCA: Calculation rules
3.1 Declared unit
In accordance with the PCR B 1 m2 membrane is chosen as the declared unit.
Product Unit Value
Declared Unit m2 membrane 1
Unit weight g/m2 203
Conversion factor to 1 kg - 4.93
3.2 System boundary
The EPD is a complete life cycle with a functional unit. It considers all potential environmental impacts
of the product from the cradle to the end of life. Table under LCA:Results provides an overview of the
information modules or product life cycle phases considered in the LCA. The manufacturing phase in-
cludes the production or extraction and processing of raw materials, the transport to the respective
production plant and the production of the waterproofing membrane. All inputs (raw materials, pre-
cursors, energy, and auxiliary materials) as well as the by-products and waste are considered for all life
cycle phases. Finally, only production-related energy consumption (excluding administration and social
rooms) is considered.
The year 2021 represents the time reference for raw materials and electricity consumption. Due to the
production location Germany is considered as the geographical reference area. However, environmen-
tal effects such as the greenhouse effect can occur with a strong spatial and temporal offset.
The following production steps are considered during the manufacturing phase:
• Extraction and processing of the raw materials (PP non-woven, LDPE granulate, PE colour
batch, colour, diluent)
• Transport to the production site
• Processing of the products (extrusion, printing, assembly, finishing)
• Packaging (including packaging material)
• End-of-life (including transport)
Secondary fuels are not included in the production process and are therefore not considered. The
waste materials and quantities produced are included in the respective modules.
3.3 Estimates and assumptions
All datasets chosen for the LCA refer to the EU as the geographic reference. Transport distances for all
raw materials used (raw materials, operating materials, packaging) could be recorded. A payload factor
of 50 percent was used for all truck transports (suppliers, disposal transports and internal transports),
which corresponds to a full delivery and empty return trip. A data set for a non-specific truck was used
for phase A2. For the end-of-life waste scenario 100% landfilling has been assumed. The end-of-life
waste scenario per input material has been chosen and for each row material 100% landfilling has been
modeled. No CO certificates were considered.
2
Page | 6 BOSTIK AB – Tätskiktsfolie Pro LX
3.4 Cut-off criteria
All flows that are relevant for the production of the waterproofing membrane were recorded. All pro-
cess specific data could be determined and modelled using generic data (EcoInvent 3.6).
3.5 Period under review
All process-specific data was collected for the operating year 2021. The quantities of raw materials as
well as energy consumption have been recorded and averaged over the entire operating year 2021.
3.6 Data quality
For all processes primary data was collected and provided by BOSTIK AB. The primary data refers to
year 2021. For the data, which is not influenced by the manufacturer, generic data was used. The sec-
ondary data was taken from the database EcoInvent (version 3.6, 2019). The database is maintained
on a regular basis and thus meets the requirements of EN 15804 (background data not older than 10
years). The power sources were chosen from data for the Germany in 2021, in accordance with the
geographical and time representativeness. The data quality is very good, because all process specific
data could be documented and modelled by using the generic data.
RETHiNK EPD web application from the company NIBE was used to model the life cycle for the pro-
duction and disposal of the declared product systems. To ensure that the results are comparable, con-
sistent background data from the international database EcoInvent was used in the LCA (e.g. data rec-
ords on energy, transport, auxiliary materials, and supplies). Almost all consistent data sets contained
in the EcoInvent database are documented and can be viewed online.
3.7 Allocation
Allocations were avoided as far as possible. There are no coproducts or byproduct in the manufactur-
ing of the waterproofing membrabne. Based on energy consumption measurements, the energy
demand was allocated to the individual products. Recyclebare production waste is collected and sold
to the third party.
3.8 Comparability
In principle, a comparison or assessment of the environmental impacts of different products is only
possible if they have been prepared in accordance with EN 15804. For the evaluation of the
comparability, the following aspects have to be considered in particular: PCR used , functional or
declared unit, geographical reference, definition of the system boundary, declared modules, data
selection (primary or secondary data, background database, data quality), scenarios used for use and
disposal phases, and the life cycle inventory (data collection, calculation methods, allocations, validity
period). PCRs and general program instructions of different EPDs programs may differ. A comparability
needs to be evaluated. For further guidance see EN 15804+A2 (5.3 Comparability of EPD for
construction products) and ISO 14025 (6.7.2 Requirements for comparability).
Page | 7 BOSTIK AB – Tätskiktsfolie Pro LX
4. LCA: Scenarios and additional technical information
The distance between the production and the construction site (Module A4) was calculated based on
the sold products in 2021. Accordingly, it was calculated the product was partially distributed by road
(536 km) and partially by ship. As means of transportation truck (unspecified) and transoceanic freight
ship were chosen.
The installation of the waterproofing membrane is usually conducted manually. A reject or unused
portion of 7% of the waterproofing membrane is assumed during the installation process (Module A5).
For the Module C1 (demolition) it has been assumed that it can be considered irrelevant, because no
significant additional energy is needed for the demolition of waterproofing membrane within an ap-
plied system. E.g., if the waterproofing membrane is applied under tiles, the demolition energy for the
removal of tiles will not be considerably higher if the waterproofing membrane is applied underneath.
The end-of-life waste scenario per input material has been chosen and for each row material 100%
landfilling has been modeled under the consideration of suitable loads and benefits.
Note: The transport distances of the waste are based on the standard waste scenarios of the NMD
Determination Method (SBK 2019): incineration 150 km/ recycling 50 km / landfill 100 km; vehicle:
truck, unspecific. According the EN 15804, loads are credited in Modules A3 or C3 to C4 and benefits
are credited in module D.
For all road transports, the environmental profile of a non-specific truck transport was used (conserva-
tive assumption): The vehicle operates with diesel, and it provides a fleet average that includes differ-
ent lorry classes as well as EURO classes. This environmental profile contains data for transport, which
is calculated for an average load factor, including empty return trips (EcoInvent 3.6).
5. LCA: Results
The following tables show the results of the impact assessment indicators, resource use, waste and
other output streams. The results presented here refer to the declared specific product.
Disclaimer on ADP-e, ADP-f, WDP, ETP-fw, HTP-c, HTP-nc, SQP: The results of these environmental
impact indicators must be used with caution, as the uncertainties in these results are high or as there
is limited experience with the indicator.
Disclaimer on IR: This impact category mainly addresses the potential effect of low dose ionizing radi-
ation on human health in the nuclear fuel cycle. It does not consider effects due to possible nuclear
accidents and occupational exposures, nor does it consider radioactive waste disposal in underground
facilities. Potential ionizing radiation from soil, radon, and some building materials is also not meas-
ured by this indicator.
Page | 8 BOSTIK AB – Tätskiktsfolie Pro LX
Description of the system boundary
Benefits and loads beyond
Product stage Construction process stage Use stage End of life stage
the system boundaries
la ire ta m w a Ry lp p u s tro p s n a rT u n a M-g n iru tc a f tro p s n a rTu n a m m o r- f o t re ru tc a fe s u fo e c a lp n o itc u rts n o C- n o ita lla ts n is s e c o rp e s U e c n na in a Me t- ria p e R tn e m e c a lp e R n e m ruh fs ei Rb - la n o ita re p Oe s u y g re n e la n o ita re p Oe s u re ta w e D- / n o itc u rts n o cn o itilo m e d tro p s n a rT e ts a Wg n is s e c o rp la s o p s iD y re ev o s uc ee R -- g n ilc y c e R- a itn e to pl
R
A1 A2 A3 A4 A5 B1 B2 B3 B4 B5 B6 B7 C1 C2 C3 C4 D
X X X X X MND MND MND MND MND MND MND X X X X X
X=Module declared | MND=Module not declared
Results of the LCA – Environmental impact: 1 m2 Tätskiktsfolie Pro LX
Parameter Unit A1 A2 A3 A4 A5 C1 C2 C3 C4 D
Core environmental impact indicators (EN 15804+A2)
ADP-mm kg Sb eq. 5,04E-06 2,04E-07 1,81E-06 4,01E-07 5,56E-07 0,00E+00 6,67E-08 0,00E+00 2,21E-08 -5,47E-08
ADP-f MJ 1,52E+01 1,22E-01 2,78E+00 2,39E-01 1,34E+00 0,00E+00 3,97E-02 0,00E+00 4,89E-02 -1,99E-01
AP mol H+ eq. 1,70E-03 4,68E-05 7,83E-04 9,54E-05 1,94E-04 0,00E+00 1,53E-05 0,00E+00 1,80E-05 -3,52E-05
EP-fw kg PO4 eq. 1,11E-05 8,13E-08 2,95E-05 1,60E-07 2,91E-06 0,00E+00 2,65E-08 0,00E+00 3,69E-08 -2,11E-07
EP-m kg N eq. 2,84E-04 1,65E-05 1,62E-04 3,31E-05 3,83E-05 0,00E+00 5,38E-06 0,00E+00 1,05E-05 -8,41E-06
EP-t mol N eq. 3,15E-03 1,82E-04 2,11E-03 3,65E-04 4,43E-04 0,00E+00 5,93E-05 0,00E+00 6,63E-05 -1,16E-04
GWP-b kg CO2 eq. 7,97E-04 3,72E-06 1,29E-02 7,21E-06 7,34E-03 0,00E+00 1,21E-06 0,00E+00 2,22E-05 1,85E-02
GWP-f kg CO2 eq. 4,58E-01 8,06E-03 2,00E-01 1,59E-02 5,36E-02 0,00E+00 2,63E-03 0,00E+00 2,72E-02 -6,88E-03
GWP-luluc kg CO2 eq. 2,38E-04 2,95E-06 7,35E-04 5,89E-06 6,96E-05 0,00E+00 9,64E-07 0,00E+00 1,01E-06 -1,69E-05
GWP-total kg CO2 eq. 4,59E-01 8,07E-03 2,14E-01 1,59E-02 6,10E-02 0,00E+00 2,63E-03 0,00E+00 2,72E-02 1,16E-02
ODP kg CFC 11 eq. 1,23E-08 1,78E-09 1,01E-08 3,51E-09 2,13E-09 0,00E+00 5,81E-10 0,00E+00 6,39E-10 -4,99E-10
POCP kg NMVOC eq. 1,74E-03 5,19E-05 4,34E-04 1,04E-04 1,77E-04 0,00E+00 1,69E-05 0,00E+00 2,50E-05 -3,56E-05
WDP m3 world eq. 4,41E-01 4,35E-04 4,34E-02 8,53E-04 3,54E-02 0,00E+00 1,42E-04 0,00E+00 2,10E-03 -4,68E-03
Additional environmental impact indicators (EN 15804+A2)
ETP-fw CTUe 3,10E+00 1,08E-01 3,16E+00 2,13E-01 5,26E-01 0,00E+00 3,54E-02 0,00E+00 5,10E-02 -1,77E-01
HTP-c CTUh 1,19E-10 3,52E-12 8,34E-11 6,97E-12 1,86E-11 0,00E+00 1,15E-12 0,00E+00 1,38E-12 -3,13E-12
HTP-nc CTUh 3,36E-09 1,19E-10 2,31E-09 2,33E-10 4,60E-10 0,00E+00 3,87E-11 0,00E+00 3,34E-11 -1,00E-10
IRP kBq U235 eq. 1,48E-02 5,09E-04 9,05E-03 1,00E-03 1,85E-03 0,00E+00 1,66E-04 0,00E+00 1,91E-04 -1,95E-04
PM disease incidence 1,32E-08 7,25E-10 5,57E-09 1,42E-09 1,60E-09 0,00E+00 2,37E-10 0,00E+00 3,40E-10 -3,68E-10
SQP 8,14E-01 1,05E-01 8,77E+00 2,06E-01 6,99E-01 0,00E+00 3,44E-02 0,00E+00 1,16E-01 -1,79E+00
Page | 9 BOSTIK AB – Tätskiktsfolie Pro LX
ADP-mm=Depletion of abiotic resources - minerals and metals| ADP-f=Depletion of abiotic resources - fossil fuels | AP=Acidification potential | EP-fw=Eutrophication, freshwater | EP-m=Eutrophication, marine | EP-t=Eutrophication, terrestrial | GWP-b=Global warming
potential - biogenic | GWP-f=Global warming potential - fossil | GWP-luluc=Global warming potential - land use and land use change |GWP-total=Global warming potential |ODP=Ozone depletion |POCP=Photochemical ozone formation | WDP=Water use | ETP-fw=Ecotox-
icity, freshwater | HTP-c=Human toxicity, cancer effects | HTP-nc=Human toxicity, non-cancer effects| IRP=Ionising radiation, human health | PM= disease in-cidence | SQP=Land use related impacts (Potential Soil quality index)
Results of the LCA – Resource use and environmental information: 1 m2 Tätskiktsfolie Pro LX
Parameter Unit A1 A2 A3 A4 A5 C1 C2 C3 C4 D
PERE MJ 3,85E-01 1,52E-03 1,82E+00 2,99E-03 1,56E-01 0,00E+00 4,97E-04 0,00E+00 3,30E-03 -1,09E-01
PERM MJ 0,00E+00 0,00E+00 3,61E-01 0,00E+00 2,52E-02 0,00E+00 0,00E+00 0,00E+00 0,00E+00 -2,22E-01
PERT MJ 3,85E-01 1,52E-03 2,19E+00 2,99E-03 1,82E-01 0,00E+00 4,97E-04 0,00E+00 8,61E-04 -3,31E-01
PENRE MJ 8,93E+00 1,29E-01 2,90E+00 2,54E-01 8,72E-01 0,00E+00 4,21E-02 0,00E+00 7,21E-02 -1,26E-01
PENRM MJ 7,41E+00 0,00E+00 5,12E-02 0,00E+00 5,43E-01 0,00E+00 0,00E+00 0,00E+00 0,00E+00 -8,76E-02
PENRT MJ 1,63E+01 1,29E-01 2,98E+00 2,54E-01 1,43E+00 0,00E+00 4,21E-02 0,00E+00 5,20E-02 -2,14E-01
SM Kg 0,00E+00 0,00E+00 0,00E+00 0,00E+00 0,00E+00 0,00E+00 0,00E+00 0,00E+00 0,00E+00 0,00E+00
RSF MJ 0,00E+00 0,00E+00 0,00E+00 0,00E+00 0,00E+00 0,00E+00 0,00E+00 0,00E+00 0,00E+00 0,00E+00
NRSF MJ 0,00E+00 0,00E+00 0,00E+00 0,00E+00 0,00E+00 0,00E+00 0,00E+00 0,00E+00 0,00E+00 0,00E+00
FW m³ 6,96E-03 1,48E-05 2,21E-03 2,91E-05 6,74E-04 0,00E+00 4,83E-06 0,00E+00 5,11E-05 -6,88E-05
HWD Kg 2,16E-06 3,08E-07 4,07E-06 6,04E-07 5,26E-07 0,00E+00 1,01E-07 0,00E+00 7,44E-08 -9,05E-08
NHWD Kg 2,06E-02 7,71E-03 1,88E-02 1,51E-02 1,81E-02 0,00E+00 2,52E-03 0,00E+00 1,95E-01 -5,77E-04
RWD Kg 1,26E-05 7,98E-07 1,11E-05 1,57E-06 1,90E-06 0,00E+00 2,61E-07 0,00E+00 2,91E-07 -2,02E-07
CRU Kg 0,00E+00 0,00E+00 0,00E+00 0,00E+00 0,00E+00 0,00E+00 0,00E+00 0,00E+00 0,00E+00 0,00E+00
MFR Kg 0,00E+00 0,00E+00 7,87E-03 0,00E+00 1,89E-02 0,00E+00 0,00E+00 0,00E+00 0,00E+00 0,00E+00
MER Kg 0,00E+00 0,00E+00 0,00E+00 0,00E+00 0,00E+00 0,00E+00 0,00E+00 0,00E+00 0,00E+00 0,00E+00
EE MJ 0,00E+00 0,00E+00 0,00E+00 0,00E+00 0,00E+00 0,00E+00 0,00E+00 0,00E+00 0,00E+00 7,01E-02
PERE=renewable primary energy ex. raw materials | PERM=renewable primary energy used as raw materials | PERT=renewable primary energy total | PENRE=non-renewable primary energy ex. raw materials | PENRM=non-renewable
primary energy used as raw materials | PENRT=non-renewable primary energy total | SM=use of secondary material | RSF=use of renewable secondary fuels | NRSF=use of non-renewable secondary fuels | FW=use of net fresh water |
HWD=hazardous waste disposed | NHWD=non-hazardous waste disposed | RWD=radioactive waste disposed | CRU=Components for re-use | MFR=Materials for recycling | MER=Materials for energy recovery | EE=Exported energy
Page | 10 BOSTIK AB – Tätskiktsfolie Pro LX
6. LCA: Interpretation
As shown in the figure below, A1 (raw material supply) and A3 (manufacturing) dominate in most
environmental core indicators. The highest impact (app. 50%) on the GWP is attributed to the LDPE
granulate, followed by the PP non-woven (app. 27%). Among energy inputs the highest contribution
to the GWP is caused by the cooling process (11%). Transports A2 and C2 have only a minor impact
within all core indicators, whereas the transport to the customers (A4) has a slightly bigger impact
compared to other two transports. The installation phase (A5) contributes with around 8-10% to each
environmental category. However, this phase is strongly dependent on the 7% construction waste
assumption. Since the product is completely landfilled after reaching the end-of-life credits beyond the
system boundaries (module D) are mainly originating from the packaging material.
100%
80%
60%
40%
20%
0%
-20%
A1 A2 A3 A4 A5 C1 C2 C3 C4 D
Figure 2: Tätskiktsfolie Pro LX - Impact of the individual modules on the environmental core indicators
The data quality can be classified as good overall. All relevant process-specific data could be collected
in the operational data collection. Consistent data sets from the EcoInvent database (version 3.6) were
available for almost all inputs and outputs. The background data meet the requirements of EN 15804,
and the production data were recorded for the 2021 operating year. The quantities of raw materials
and supplies used as well as energy consumption were recorded for the entire operating year.
Page | 11 BOSTIK AB – Tätskiktsfolie Pro LX
7. References
BNB Service Life of Building Components, https://www.nachhaltigesbauen.de/aus-
tausch/nutzungsdauern-von-bauteilen/, last assessed 2022-07-01
CML-IA April 2013 – Charakterisierungsfaktoren entwickelt durch Institut of Environmental Sciences
(CML): Universität Leiden, Niederlande - http://www.cml.leiden.edu/software/data-cmlia.html
Donndorf, R., Kahle H., Müller, G., Philipp H-J., Taschow, H-J., Wolf, O. (1973): Werkstoffeinsatz und
Korrosionsschutz in der chemischen Industrie. VEB Deutscher Verlag für Grundstoffindustrie Leipzig.
European Commission Joint Research Centre Institute for Prospective Technological Studies (JCR
2014): End-of-waste criteria for waste plastic for conversion, Seville, 2014, doi:10.2791/13033
Klöpffer, W., Grahl B.: Ökobilanz (LCA) – Ein Leitfaden für die Ausbildung und Beruf, Wily-VCH Ver-lag,
Weinheim, 2007
Rosauer, V. (2010): Abschätzung der herstellungsbedingten Qualität und Lebensdauer von Asphalt-
deckschichten mit Hilfe der Risikoanalyse (Estimation of the production-related quality and service life
of asphalt wearing courses with the aid of risk analysis). Technischen Universität Darmstadt, 2010
Protocol EPD-online - 25011.16.03.015 - Protocol EPD online - NMD, version 1.2, November 2016, NIBE
Standards and laws
ISO 14040:2006, Environmental management - Life cycle assessment - Principles and framework
ISO 14044:2006, Environmental management - Life cycle assessment - Requirements and guide-lines
ISO 14025:2006: Environmental labels and declarations — Type III environmental declarations — Prin-
ciples and procedures EN 13249
EN 15804:2012+A1:2019: Sustainability of construction works — Environmental Product Declarations
— Core rules for the product category of construction products
EN 15804:2012+A2:2019 Sustainability of construction works — Environmental Product Declarations
— Core rules for the product category of construction products
PCR A: General Program Category Rules for Construction Products from the EPD program Kiwa-Ecobil-
ity Experts, R.0_2021-07-16
PCR B: Product Category Rules (PCR) from the Kiwa-Ecobility Experts EPD program: “Product Category
Rules for plastic and rubber sheets for roof and wall waterproofing”, edition 2021-12-28 (draft)
Page | 12 BOSTIK AB – Tätskiktsfolie Pro LX
Publisher E-mail DE.Ecobility.Experts@kiwa.com
Kiwa-Ecobility Experts Web https://www.kiwa.com/de/de/th
Voltastr. 5 emes/ecobility-experts/ecobility-
13355 Berlin experts/
Germany
Programme operator E-mail DE.Ecobility.Experts@kiwa.com
Kiwa-Ecobility Experts Web https://www.kiwa.com/de/de/th
Voltastr. 5 emes/ecobility-experts/ecobility-
13355 Berlin experts/
Germany
Author of the Life Cycle Tel. +49 (0)30 467761-43
Assessment Fax. +49 (0)30 467761-10
Kiwa GmbH E-mail DE.Nachhaltigkeit@kiwa.com
Voltastr. 5 Web https://www.kiwa.com/
13355 Berlin
Germany
Owner of the declaration Tel. + 46 (0)42 19 50 00
BOSTIK AB E-mail info.se@bostik.com
Strandbadsvägen 22 Web https://www.bostik.com/
251 09 Helsingborg
Sweden
Kiwa-Ecobility Experts is
established member of the
Page | 13 BOSTIK AB – Tätskiktsfolie Pro LX
