Environmental product declaration
in accordance with ISO 14025 and EN 15804+A2
BUD Stack
Owner of the declaration: Program operator:
Fora Form AS The Norwegian EPD Foundation
Product: Declaration number:
BUD Stack
Registration number:
Declared unit:
1 pcs Issue date:
10.04.2024
This declaration is based on Product Category Rules:
CEN Standard EN 15804:2012+A2:2019 serves as core Valid to:
PCR
The Norwegian EPD Foundation EPD software:
NPCR 026:2022 Part B for Furniture
LCAno EPD generator ID: 198841
1 / 12
General information
Product Owner of the declaration:
BUD Stack Fora Form AS
Contact person: Kåre Sætre
Phone: +47 700 46 000
e-mail: info@foraform.com
Program operator: Manufacturer:
The Norwegian EPD Foundation Fora Form AS
Post Box 5250 Majorstuen, 0303 Oslo, Norway
Phone: +47 977 22 020
web: www.epd-norge.no
Declaration number: Place of production:
Fora Form AS
Mosflatevegen
6154 Ørsta, Norway
This declaration is based on Product Category Rules: Management system:
CEN Standard EN 15804:2012+A2:2019 serves as core PCR NS-EN ISO 14001: 2015 No. 800406.NS-EN ISO 9001: 2015 No.
NPCR 026:2022 Part B for Furniture 901268.NS-EN ISO 45001: 2018 No 907167.
Statement of liability: Organisation no:
The owner of the declaration shall be liable for the underlying 986 581 421
information and evidence. EPD Norway shall not be liable with respect
to manufacturer information, life cycle assessment data and
evidences.​
Declared unit: Issue date:
1 pcs BUD Stack 10.04.2024
Declared unit (cradle to gate) with option: Valid to:
A1-A3,A4,A5,B1,B2,C1,C2,C3,C4,D
Year of study:
2024
Functional unit: Comparability:
Production of one furniture solution provided and maintained for a EPD of construction products may not be comparable if they not
period of 15 years. comply with EN 15804 and seen in a building context.
General information on verification of EPD from EPD tools: Development and verification of EPD:
Independent verification of data, other environmental information The declaration is created using EPD tool lca.tools ver EPD2022.03,
and the declaration according to ISO 14025:2010, § 8.1.3 and § 8.1.4. developed by LCA.no. The EPD tool is integrated in the company's
Verification of each EPD is made according to EPD-Norway’s management system, and has been approved by EPD Norway.
guidelines for verification and approval requiring that tools are i)
integrated into the company's environmental management system, ii) Developer of EPD: Kåre Sætre
the procedures for use of the EPD tool are approved by EPD-Norway,
Reviewer of company-specific input data and EPD: Katrine Østgaard
and iii) the process is reviewed annually by an independent third
party verifier. See Appendix G of EPD-Norway's General Programme
Instructions for further information on EPD tools
Verification of EPD tool: Approved:
Independent third party verification of the EPD tool, background data
and test-EPD in accordance with EPDNorway's procedures and
guidelines for verification and approval of EPD tools.
Håkon Hauan, CEO EPD-Norge
Third party verifier:
Elisabet Amat, GREENIZE projects
(no signature required)
2 / 12
Product
Product description:
BUD is the playful chair for the meeting rooms, dining area or as a visual element in informal social zones.
BUD was created to give playful and modern environments a chair that differs from the traditional.
BUD brings FUN back into zones and spaces where different people come together to create.
It has a low back that makes it easy to communicate, while its round and open design makes it stand out in the crowd.
With BUD, you get a playful friend who makes it easy to enjoy yourself.
Product specification
The chair is assembled in Ørsta, Norway.
Steel parts contains between 15-36% recycled scrap steel
Backrest and seat is made of flexible molded polyurethane foam. Cold cured.
Plywood’s formaldehyde emission level is significantly below EN 13986 Class E1 and it is complying to EPA TSCA Title VI and CARB Phase 2.
Powder coating consists of prime-cured polyester pre-treatment with biological degreasing for high quality adhesion
Chair variants:
BUD Stack: Four leg stacking w/plastic gliders (stacks 3 chairs, not to be stacked over time)
BUD Rotate: Four leg with auto return swivel and plastic glides
BUD Unite: Star base with 360 degres swivel, tilt mechanism and wheels with soft rolling
BUD Meet: Star base with 360 degres swivel, tilt mechanism and plastic glides
Recycled share in Recycled share in
Materials kg %
material (kg) material (%)
Metal - Steel 3,69 47,25 0,74 20,00
Plastic - Acrylonitrile butadiene styrene (ABS) 0,25 3,20 0,00 0,00
Plastic - Polyoxymethylene (POM) 0,04 0,51 0,00 0,00
Plastic - Polyurethane (PUR) 1,65 21,13 0,00 0,00
Powder coating 0,04 0,51 0,00 0,00
Textile - Wool 0,54 6,91 0,00 0,00
Wood - Plywood 1,60 20,49 0,00 0,00
Total 7,81 0,74
Recycled share in Recycled share in
Packaging kg %
material (kg) material (%)
Packaging - Cardboard 0,40 20,00 0,00 0,00
Recycled cardboard 1,60 80,00 1,60 100,00
Total incl. packaging 9,81 2,34
Technical data:
Width 68cm
Height 77cm
Depth 58cm
Seat height 48 cm
Weight 7,81 kg
The seating furniture is tested and meets the requirements for strength and safety according to: EN 16139:2013 / EN 1022:2023 / EN
16139:2013 Test level 1
Market:
Worldwide
Reference service life, product
15 years
Reference service life, building
15 years
3 / 12
LCA: Calculation rules
Declared unit:
1 pcs BUD Stack
Cut-off criteria:
All major raw materials and all the essential energy is included. The production processes for raw materials and energy flows with very small
amounts (less than 1%) are not included. These cut-off criteria do not apply for hazardous materials and substances.
Allocation:
The allocation is made in accordance with the provisions of EN 15804. Incoming energy and water and waste production in-house is allocated
equally among all products through mass allocation. Effects of primary production of recycled materials is allocated to the main product in which
the material was used. The recycling process and transportation of the material is allocated to this analysis.
Data quality:
Specific data for the product composition are provided by the manufacturer. They represent the production of the declared product and were
collected for EPD development in the year of study. Background data is based on registered EPDs according to EN 15804, Ostfold Research
databases, ecoinvent and other LCA databases. The data quality of the raw materials in A1 is presented in the table below.​
Materials Source Data quality Year
Metal - Steel ecoinvent 3.6 Database 2019
Packaging - Cardboard Modified ecoinvent 3.6 Database 2019
Plastic - Acrylonitrile butadiene styrene (ABS) ecoinvent 3.6 Database 2019
Plastic - Polyoxymethylene (POM) ecoinvent 3.6 Database 2019
Plastic - Polyurethane (PUR) ecoinvent 3.6 Database 2019
Powder coating Ecoinvent 3.6 Database 2019
Recycled cardboard Modified ecoinvent 3.6 Database 2019
Textile - Wool Modified ecoinvent 3.6 Database 2019
Wood - Plywood modified ecoinvent 3.6 Database 2019
4 / 12
System boundaries (X=included, MND=module not declared, MNR=module not relevant)
Construction Beyond the system
Product stage Use stage End of life stage
installation stage boundaries
A1 A2 A3 A4 A5 B1 B2 B3 B4 B5 B6 B7 C1 C2 C3 C4 D
X X X X X X X MND MND MND MND MND X X X X X
System boundary:
Additional technical information:
We want you to enjoy your furniture for many years to come. If you follow our advice in our’s Quality and Maintenance manual you contribute to
prolonged life of your furniture. We use as far as possible environmentally friendly materials and processes in our manufacturing unit in Ørsta
Norway. Our goal is to manufacture furniture that can last for generations. All furniture made by Fora Form are made of FSC certified wood,
manufactured according to ISO 14001, and has an EPD on all products. This ensures sustainability and a “cradle to cradle” philosophy. We actively
work to reduce waste. All pa For a Form collaborate with Norsk Gjenvinning and Grønt Punkt (Green Dot Norway plc) regarding recycling of used
packing materials. All wood is FSC certified.
Norwegian and Swedish Møbelfakta are accredited test facilities where furniture quality, strength, durability, flammability, safety, emissions and
materials are tested and documented. A piece of furniture, which lives up to the three areas of requirements of Møbelfakta, has undergone
extensive testing, is produced according to ethical guidelines and has been approved according to environmental requirements. Møbelfakta is an
guarantee of high quality products.
Almost all of Fora Forms collection is Møbelfakta approved.
Fora Form are ISO 9001 quality management,ISO 14001 environmental management and ISO 45001 occupational health and safety management
certified.
Sustainability is important for Fora Form.
Our manufacturing unit in Ørsta use as far as possible electricity that is 100% originated from renewable sources. Alternatively Norwegian mix
Transportation to an average customer in Oslo is 540 km
waR slairetam tropsnarT gnirutcafunaM tropsnarT ylbmessA e​sU ecnanetniaM riapeR tnemecalpeR tnemhsibrufeR lanoitarepO ygrene esu lanoitarepO esu retaw -eD noitcurtsnoc noitilomed tropsnarT etsaW gnissecorp lasopsiD -yrevoceR-esueR laitnetop-gnilcyceR
5 / 12
LCA: Scenarios and additional technical information
The following information describe the scenarios in the different modules of the EPD.
Capacity utilisation Value
Transport from production place to user (A4) Distance (km) Fuel/Energy Consumption Unit
(incl. return) % (Liter/tonne)
Truck, 16-32 tonnes, EURO 6 (km) 36,7 % 540 0,043 l/tkm 23,22
Assembly (A5) Unit Value
Waste, packaging, cardboard, 100 % recycled, to
kg 1,60
average treatment (kg)
Waste, packaging, corrugated board box, 0 %
kg 0,40
recycled, to average treatment (kg)
Maintenance (B2) Unit Value
Water, tap water (kg) kg/DU 1,00
Capacity utilisation Value
Transport to waste processing (C2) Distance (km) Fuel/Energy Consumption Unit
(incl. return) % (Liter/tonne)
Truck, 7.5-16 tonnes, HVO, EURO 6 (kgkm) 35,4 % 85 0,056 l/tkm 4,76
Waste processing (C3) Unit Value
Waste treatment per kg Non-hazardous waste,
kg 0,04
incineration with fly ash extraction - C3 (kg)
Waste treatment per kg Plastics, Mixture,
kg 0,25
municipal incineration with fly ash extraction (kg)
Waste treatment per kg Polyoxymethylene (POM),
kg 0,04
incineration with fly ash extraction (kg) - CH - C3
Waste treatment per kg Polyurethane (PU),
kg 1,65
incineration (kg)
Waste treatment per kg Scrap steel, incineration
kg 3,69
with fly ash extraction (kg)
Waste treatment per kg Textile, incineration with
kg 0,54
fly ash extraction (kg)
Waste treatment per kg Wood, incineration with
kg 1,60
fly ash extraction (kg)
Waste, materials to recycling (kg) kg 1,25
Disposal (C4) Unit Value
Landfilling of ashes and residues from
kg 2,44
incineration of Scrap steel (kg)
Landfilling of ashes from incineration of Non-
hazardous waste, process per kg ashes and kg 0,01
residues - C4 (kg)
Landfilling of ashes from incineration of Plastics,
Mixture, municipal incineration with fly ash
kg 0,01
extraction, process per kg ashes and residues - C4
(kg)
Landfilling of ashes from incineration of
Polyoxymethylene (POM), process per kg ashes kg 0,00
and residues (kg) - CH - C4
Landfilling of ashes from incineration of
Polyurethane (PU), process per kg ashes and kg 0,06
residues - C4 (kg)
Landfilling of ashes from incineration of Textile,
kg 0,03
soiled, process per kg ashes and residues (kg)
Landfilling of ashes from incineration of Wood,
kg 0,02
process per kg ashes and residues (kg)
Benefits and loads beyond the system
Unit Value
boundaries (D)
Substitution of electricity, in Norway (MJ) MJ 4,37
Substitution of primary steel with net scrap (kg) kg 1,00
Substitution of thermal energy, district heating, in
MJ 66,13
Norway (MJ)
6 / 12
LCA: Results
The LCA results are presented below for the declared unit defined on page 2 of the EPD document.
Environmental impact
Indicator Unit A1-A3 A4 A5 B1 B2 C1 C2 C3 C4 D
GWP-total
kg CO2 -
6,08E+01 6,89E-01 3,43E+00 0 3,46E-04 0 3,50E-02 8,71E+00 3,24E-02 -1,50E+00
eq
GWP-fossil
kg CO2 -
4,79E+01 6,89E-01 3,24E-02 0 3,43E-04 0 3,48E-02 5,25E+00 3,24E-02 -1,49E+00
eq
GWP-biogenic
kg CO2 -
1,04E+01 2,85E-04 3,40E+00 0 2,16E-06 0 6,41E-05 3,46E+00 2,64E-05 -1,40E-03
eq
GWP-luluc
kg CO2 -
2,47E+00 2,45E-04 1,07E-05 0 5,59E-07 0 6,35E-05 3,72E-05 8,97E-06 -1,37E-02
eq
kg
ODP CFC11 - 3,06E-06 1,56E-07 6,83E-09 0 3,00E-11 0 5,98E-09 2,73E-08 8,92E-09 -2,79E-02
eq
mol H+
AP 8,15E-01 1,98E-03 1,53E-04 0 2,00E-06 0 2,40E-04 4,41E-03 2,10E-04 -8,64E-03
-eq
EP-FreshWater kg P -eq 8,26E-03 5,50E-06 2,66E-07 0 2,74E-08 0 1,41E-06 2,39E-06 3,42E-07 -1,02E-04
EP-Marine kg N -eq 1,41E-01 3,92E-04 5,07E-05 0 3,18E-07 0 5,94E-05 2,41E-03 7,39E-05 -2,17E-03
mol N -
EP-Terrestial 2,93E+00 4,38E-03 5,49E-04 0 3,70E-06 0 6,68E-04 2,33E-02 8,21E-04 -2,28E-02
eq
kg
POCP NMVOC 1,72E-01 1,68E-03 1,58E-04 0 1,16E-06 0 2,43E-04 5,57E-03 2,35E-04 -8,60E-03
-eq
ADP- kg Sb-
1,17E-03 1,90E-05 7,87E-07 0 9,59E-09 0 5,30E-06 1,07E-06 4,96E-07 -2,28E-05
minerals&metals1 eq
ADP-fossil1 MJ 6,16E+02 1,04E+01 4,53E-01 0 5,86E-03 0 7,12E-01 2,23E+00 6,66E-01 -1,48E+01
WDP1 m3 1,75E+03 1,01E+01 5,74E-01 0 1,04E-01 0 2,57E+00 6,58E+00 1,73E+00 -1,11E+01
GWP-total = Global Warming Potential total; GWP-fossil = Global Warming Potential fossil fuels; GWP-biogenic = Global Warming Potential biogenic; GWP-luluc =
Global Warming Potential land use and land use change; ODP = Depletion potential of the stratospheric ozone layer; AP = Acidification potential, Accumulated
Exceedance; EP-freshwater = Eutrophication potential, fraction of nutrients reaching freshwater end compartment: EP-marine = Eutrophication potential, fraction of
nutrients reaching marine end compartment; EP-terrestrial = Eutrophication potential, Accumulated Exceedance; POCP = Formation potential of tropospheric ozone;
ADP-minerals&metals = Abiotic depletion potential for non-fossil resources; ADP-fossil = Abiotic depletion for fossil resources potential; WDP = Water (user)
deprivation potential, deprivation-weighted water consumption
"Reading example: 9,0 E-03 = 9,0*10-3 = 0,009"
*INA Indicator Not Assessed
1. The results of this environmental impact indicator shall be used with care as the uncertainties on these results are high or as there is limited experienced with the
indicator
Remarks to environmental impacts
The product meets the requirements for low emissions.
7 / 12
Additional environmental impact indicators
Indicator Unit A1-A3 A4 A5 B1 B2 C1 C2 C3 C4 D
PM Disease incidence 7,20E-06 4,22E-08 2,26E-09 0 1,70E-11 0 6,64E-09 2,22E-08 3,73E-09 -2,83E-07
IRP2 kgBq U235 -eq 1,74E+00 4,55E-02 1,94E-03 0 4,05E-05 0 2,34E-03 3,77E-03 2,70E-03 -3,11E-02
ETP-fw1 CTUe 2,64E+03 7,72E+00 6,04E-01 0 6,35E-03 0 1,11E+00 1,46E+01 4,55E-01 -9,13E+01
HTP-c1 CTUh 1,27E-07 0,00E+00 1,80E-11 0 1,00E-12 0 0,00E+00 5,65E-10 1,80E-11 -5,85E-09
HTP-nc1 CTUh 1,97E-06 8,44E-09 7,58E-10 0 2,10E-11 0 1,99E-09 1,83E-08 5,17E-10 8,66E-08
SQP1 dimensionless -2,13E+04 7,29E+00 3,04E-01 0 1,64E-03 0 1,10E+00 2,77E-01 1,49E+00 -3,74E+01
PM = Particulate Matter emissions; IRP = Ionizing radiation – human health; ETP-fw = Eco toxicity – freshwater; HTP-c = Human toxicity – cancer effects; HTP-nc =
Human toxicity – non cancer effects; SQP = Soil Quality (dimensionless)
"Reading example: 9,0 E-03 = 9,0*10-3 = 0,009"
*INA Indicator Not Assessed
1. The results of this environmental impact indicator shall be used with care as the uncertainties on these results are high or as there is limited experienced with the
indicator
2. This impact category deals mainly with the eventual impact of low dose ionizing radiation on human health of the nuclear fuel cycle. It does not consider effects due
to possible nuclear accidents, occupational exposure nor due to radioactive waste disposal in underground facilities. Potential ionizing radiation from the soil, from
radon and from some construction materials is also not measured by this indicator.
8 / 12
Resource use
Indicator Unit A1-A3 A4 A5 B1 B2 C1 C2 C3 C4 D
PERE MJ 1,93E+02 1,49E-01 7,45E-03 0 7,95E-04 0 3,77E-02 6,84E-02 1,43E-02 -3,46E+01
PERM MJ 5,00E+01 0,00E+00 -1,57E+01 0 0,00E+00 0 0,00E+00 -3,43E+01 0,00E+00 0,00E+00
PERT MJ 2,43E+02 1,49E-01 -1,57E+01 0 7,95E-04 0 3,77E-02 -3,42E+01 1,43E-02 -3,46E+01
PENRE MJ 5,71E+02 1,04E+01 4,53E-01 0 5,87E-03 0 7,13E-01 2,24E+00 6,66E-01 -1,48E+01
PENRM MJ 6,30E+01 0,00E+00 0,00E+00 0 0,00E+00 0 0,00E+00 -6,30E+01 0,00E+00 0,00E+00
PENRT MJ 6,34E+02 1,04E+01 4,53E-01 0 5,87E-03 0 7,13E-01 -6,08E+01 6,66E-01 -1,48E+01
SM kg 2,34E+00 0,00E+00 0,00E+00 0 0,00E+00 0 0,00E+00 0,00E+00 0,00E+00 0,00E+00
RSF MJ 2,93E-01 5,33E-03 2,47E-04 0 6,39E-05 0 1,26E-03 1,59E-03 3,75E-04 3,39E-02
NRSF MJ 1,09E+00 1,91E-02 1,02E-03 0 6,30E-05 0 4,43E-03 0,00E+00 2,62E-02 -8,49E-01
FW m3 6,29E-01 1,11E-03 2,14E-04 0 1,01E-03 0 3,14E-04 7,86E-03 6,01E-04 -4,31E-02
PERE = Use of renewable primary energy excluding renewable primary energy resources used as raw materials; PERM = Use of renewable primary energy resources used
as raw materials; PERT = Total use of renewable primary energy resources; PENRE = Use of non renewable primary energy excluding non-renewable primary energy
resources used as raw materials; PENRM = Use of non renewable primary energy resources used as raw materials; PENRT = Total use of non renewable primary energy
resources; SM = Use of secondary materials; RSF = Use of renewable secondary fuels; NRSF = Use of non-renewable secondary fuels; FW = Net use of fresh water
"Reading example: 9,0 E-03 = 9,0*10-3 = 0,009"
*INA Indicator Not Assessed
9 / 12
End of life - Waste
Indicator Unit A1-A3 A4 A5 B1 B2 C1 C2 C3 C4 D
HWD kg 2,34E-01 5,37E-04 0,00E+00 0 1,11E-06 0 1,07E-04 0,00E+00 2,49E+00 -5,99E-03
NHWD kg 9,59E+00 5,07E-01 2,00E+00 0 7,12E-05 0 8,54E-02 4,00E-02 6,89E-02 -5,80E-01
RWD kg 1,72E-03 7,10E-05 0,00E+00 0 3,43E-08 0 2,75E-06 0,00E+00 4,09E-06 -2,57E-05
HWD = Hazardous waste disposed; NHWD = Non-hazardous waste disposed; RWD = Radioactive waste disposed
"Reading example: 9,0 E-03 = 9,0*10-3 = 0,009"
*INA Indicator Not Assessed
End of life - Output flow
Indicator Unit A1-A3 A4 A5 B1 B2 C1 C2 C3 C4 D
CRU kg 0,00E+00 0,00E+00 0,00E+00 0 0,00E+00 0 0,00E+00 0,00E+00 0,00E+00 0,00E+00
MFR kg 0,00E+00 0,00E+00 1,86E+00 0 0,00E+00 0 0,00E+00 1,25E+00 0,00E+00 0,00E+00
MER kg 0,00E+00 0,00E+00 2,72E-06 0 0,00E+00 0 0,00E+00 7,81E+00 0,00E+00 0,00E+00
EEE MJ 0,00E+00 0,00E+00 1,14E-01 0 0,00E+00 0 0,00E+00 4,34E+00 0,00E+00 0,00E+00
EET MJ 0,00E+00 0,00E+00 1,73E+00 0 0,00E+00 0 0,00E+00 6,56E+01 0,00E+00 0,00E+00
CRU = Components for re-use; MFR = Materials for recycling; MER = Materials for energy recovery; EEE = Exported energy electrical; EET = Exported energy thermal
"Reading example: 9,0 E-03 = 9,0*10-3 = 0,009"
*INA Indicator Not Assessed
Biogenic Carbon Content
Indicator Unit At the factory gate
Biogenic carbon content in product kg C 7,27E-01
Biogenic carbon content in accompanying packaging kg C 9,26E-01
Note: 1 kg biogenic carbon is equivalent to 44/12 kg CO2
10 / 12
Additional requirements
Greenhouse gas emissions from the use of electricity in the manufacturing phase
National production mix from import, low voltage (production of transmission lines, in addition to direct emissions and losses in grid) of applied
electricity for the manufacturing process (A3).
Electricity mix Data source Amount Unit
Electricity, European average (kWh) ecoinvent 3.6 428,03 g CO2-eq/kWh
Dangerous substances
The product contains no substances given by the REACH Candidate list.
Indoor environment
Our furniture doesn't contain any substanses that effect indoor clima
Additional Environmental Information
Key Environmental Indicators
Key environmental indicators Unit A1-A3 A4 A1-C4 A1-D
GWPtotal kg CO2 -eq 60,81 0,69 73,70 72,20
Total energy consumption MJ 765,25 10,59 780,09 729,90
Amount of recycled materials % 23,83
Additional environmental impact indicators required in NPCR Part A for construction products
Indicator Unit A1-A3 A4 A5 B1 B2 C1 C2 C3 C4 D
GWPIOBC kg CO2 -eq 6,60E+01 6,89E-01 3,24E-02 0 3,46E-04 0 3,49E-02 6,08E+00 3,51E-02 -2,04E+00
GWP-IOBC: Global warming potential calculated according to the principle of instantaneous oxidation. In order to increase the transparency of biogenic carbon
contribution to climate impact, the indicator GWP-IOBC is required as it declares climate impacts calculated according to the principle of instantaneous oxidation.
GWP-IOBC is also referred to as GWP-GHG in context to Swedish public procurement legislation.
Variants and Options
Key environmental indicators (A1-A3) for variants of this EPD
Variants Weight (kg) GWPtotal (kg CO2 -eq) Total energy consumption (MJ) Amount of recycled materials (%)
BUD Meet 11,11 103,54 1244,95 30,77
BUD Rotate 10,11 75,21 959,01 23,09
BUD Unite 11,46 104,41 1262,88 30,21
11 / 12
Bibliography
ISO 14025:2010 Environmental labels and declarations - Type III environmental declarations - Principles and procedures.
ISO 14044:2006 Environmental management - Life cycle assessment - Requirements and guidelines.
EN 15804:2012+A2:2019 Environmental product declaration - Core rules for the product category of construction products.
ISO 21930:2017 Sustainability in buildings and civil engineering works - Core rules for environmental product declarations of construction
products.
ecoinvent v3, Allocation, cut-off by classification, Swiss Centre of Life Cycle Inventories.
Iversen et al., (2021) eEPD v2021.09 Background information for EPD generator tool system verification, LCA.no Report number: 07.21
Ruud et al., (2023) EPD generator for NPCR026 Part B for Furniture - Background information for EPD generator application and LCA data,
LCA.no report number 01.23
NPCR Part A: Construction products and services. Ver. 2.0. March 2021, EPD-Norge.
NPCR 026 Part B for Furniture. Ver. 2.0 March 2022, EPD-Norge.
Program operator and publisher Phone: +47 977 22 020
The Norwegian EPD Foundation e-mail: post@epd-norge.no
Post Box 5250 Majorstuen, 0303 Oslo, Norway web: www.epd-norge.no
Owner of the declaration: Phone: +47 700 46 000
Fora Form AS e-mail: info@foraform.com
Mosflatevegen, 6154 Ørsta web: www.foraform.no
Author of the Life Cycle Assessment Phone: +47 916 50 916
LCA.no AS e-mail: post@lca.no
Dokka 6B, 1671 web: www.lca.no
Developer of EPD generator Phone: +47 916 50 916
LCA.no AS e-mail: post@lca.no
Dokka 6B,1671 Kråkerøy web: www.lca.no
ECO Platform web: www.eco-platform.org
ECO Portal web: ECO Portal
12 / 12
