ENVIRONMENTAL-PRODUCT DECLARATION
as per ISO 14025 and EN 15804+A2
Owner of the Declaration dormakaba International Holding GmbH
Publisher Institut Bauen und Umwelt e.V. (IBU)
Programme holder Institut Bauen und Umwelt e.V. (IBU)
Declaration number EPD-DOR-20210011-CCA2-EN
Issue date 11/05/2021
Valid to 10/05/2026
c-lever pro
dormakaba
www.ibu-epd.com | https://epd-online.com
General Information
dormakaba c-lever pro
Programme holder Owner of the declaration
IBU – Institut Bauen und Umwelt e.V. dormakaba International Holding GmbH
Hegelplatz 1 DORMA Platz 1
10117 Berlin 58256 Ennepetal
Germany Germany
Declaration number Declared product / declared unit
EPD-DOR-20210011-CCA2-EN 1 piece of the product: c-lever pro
This declaration is based on the product category rules: Scope:
Building Hardware products, 01/08/2021 This
(PCR checked and approved by the SVR) EPD refers to a specific product manufactured by dormakaba. The
production site is located in Wetzikon (Switzerland).
The owner of the declaration shall be liable for the underlying information
Issue date and evidence; the IBU shall not be liable with respect to manufacturer
information, life cycle assessment data and evidences.
11/05/2021
The EPD was created according to the specifications of EN 15804+A2. In
the following, the standard will be simplified as EN 15804 bezeichnet.
Valid to
10/05/2026 Verification
The standard EN 15804 serves as the core PCR
Independent verification of the declaration and data according to ISO
14025:2011
internally X externally
Dipl.-Ing Hans Peters
(chairman of Institut Bauen und Umwelt e.V.)
Florian Pronold Dr.-Ing. Wolfram Trinius,
(Managing Director Institut Bauen und Umwelt e.V.) (Independent verifier)
1 Environmental-Product Declaration - dormakaba - c-lever pro
Product
Data for Locking Cylinders acc. to the classification in EN
Product description/Product definition 1303:
The c-lever pro is an electronic door fitting. The external fitting Name Value Unit
contains an antenna and a mechatronics unit (coupling unit).
Dimensions (W X H x D) Narrow
Following identification of an authorised medium, the door can 39,8 x 298 x 21 mm
plate
be opened manually. The access authorisation is signaled
Wide plate 53,6 x 298 x 21 mm
visually but also acoustically if this option is required. The c-
lever pro is part of our comprehensive standalone portfolio Minimum bockset (with offset
35, 25 mm
dormakaba evolo. It supports the latest radio-frequency lever handles)
identification (RFID) technologies and is available with the Temperature -25 to +70 °C
wireless function: access rights are transmitted from your PC to Protection class IP55
the door components wirelessly and in real time. This offers
Humidity non-corresponding 0 to 95 %
enormous advantages in terms of security, convenience,
up to 150.000 or up to 3
programming and maintenance. Battery life at 20 °C
cylces years
Supported credential / communication technologies: Weight 1.9030 kg
Power consumption "on mode" 400 mW
• LEGIC (advant & prime)
• MIFARE (DESFire & Classic) Power consumption "idle mode" 0.08 mW
• NFC (Near Field Communication)
• Bluetooth Low Energy Power supply
This EPD covers the European and Scandinavian / Australian
versions of c-lever pro. The only difference between these - 2 batteries 1.5 V AA L91, FR6 or via the S module
versions is where the lever handle is placed. On European - via the S-module: 12–24 V AC or 12–24 V DC,
fittings it is placed above the cylinder, on ≥ 0.4
Scandinavian/Australian fittings below the cylinder. For the A
placing on the market in the European Union/European Free
Trade Association (EU/EFTA) (with the exception of The products are not harmonised in accordance with the
Switzerland) the following legal provisions apply: Construction Product Regulations (CPR) but in accordance with
other provisions for harmonisation of the EU. Compliance with
• EN 301489-1:2017-03, EN 301489-3:2017-03 the European Union Directive and technical specifications:
• EN 300330-1:2017-02, EN 300330-2:2017-02
• Radio Equipment Directive (RED) • EN 300328 V2.1.1:2016-11
• Restriction of Hazardous Substances (RoHS) • EN 300330 V2.1.1: 2017-02
• EN 301489-1 V2.2:2017-03
• EN 301489-3 V2.2:2017-03
The CE-marking considers the proof of conformity with the • EN 301489-17 V3.1.1:2017-07
respective harmonized standards based on the legal provisions • EN 50364:2010
above. For the application and use the respective national • EN 60529:2014-09
provisions apply. The provisions of the Radio Equipment Directive, RED are met.
The products are subject to CE marking according to the
Application
relevant harmonization legislation.
The c-lever pro is a mechatronical door fitting which does not
require any additional cabling (optionally available for power Base materials/Ancillary materials
supply) and offer a fully wireless, network-compatible electronic The composition of the product is the following:
locking solution with a range of functions.
Name Value Unit
Zinc 43 %
The c-lever pro range has been specially designed to fit most
standard doors and works with most European, Scandinavian Stainless Steel 28 %
and Australian mortise locks on full leaf and narrow style doors. Steel 21 %
Electronics 3 %
Possible fields of application are:
Brass 2 %
• Exterior doors Plastics 2 %
• Interior doors
Cable <0.5 %
Technical Data Paper <0.5 %
The c-lever pro has the following technical properties: Please The product includes partial articles which contain substances
list the Technical Data according to the listed in the Candidate List of REACH Regulation
List in the chapter “Product group specific calculation rules” 1907/2006/EC (date: 15.01.2019) exceeding 0.1 percentage by
mass in the alloy:
- Lead (Pb): 7439-290-1 (CAS-No.)
Example:
The main constituents of the product or its components shall be
indicated as mass percentages to enable the user of the EPD
to understand the composition of the product in delivery status.
Technical This information should support safety and efficiency during
2 Environmental-Product Declaration - dormakaba - c-lever pro
installation, use, and disposal of the product. 1) “This product/article/at least one partial article contains
substances listed in the candidate list (date: dd.mm.yyyy)
When substances from the “Candidate List of Substances of exceeding 0.1 percentage by mass: yes/no”.
Very High Concern for Authorisation” (SVHC) are part of the
formulation with a mass percentage of > 0,1 of the mass of the [if yes: List of respective SVHC and their CAS-number]
construction product, i.e. when they were added to the
formulation on purpose, then the substances shall be declared Statements like “…free of ….” and/or “…does not contain…”
including CAS-number. may not be used.
If the construction product is a substance or mixture under the
Environment and health during use
chemical law (REACH), the concentration limit value refers to
the entire product; if it is an article, the partial product or
Reference service life
component applies as a unit of reference.
The product is certified according to EN
The Candidate list can be found on the ECHA website address: 1906 and EN 16867 for 250.000 cycles. Under normal
echa.europa.eu/de/home conditions and depending on
cycle frequency, door weight etc., it means an approximate
This declaration is mandatory for all EPDs and must be duration of 10
formulated as follows: years.
LCA: Calculation rules
— A4, transport to the building site;
Declared Unit — A5, treatment of waste packaging materials arising during
The declared unit is 1 piece of the product: c-lever pro. installation into the building.
Declared unit
Use stage - Module B6
Name Value Unit
The use stage related to the operation of the building includes:
Declared unit 1 piece/product
— B6, operational energy use
Conversion factor to 1 kg (kg per declared
2.143 -
unit) End-of-life stage– Modules C1-C4 and D
The end-of-life stage includes:
For IBU core EPDs (where clause 3.6 is part of the EPD): for
— C1, de-construction, demolition:
average EPDs, an estimate of the robustness of the LCA
values must be made, e.g. concerning variability of the
— C2, transport to waste processing;
production process, geographical representativeness and the
influence of background data and preliminary products
— C3, waste processing for reuse, recovery and/or recycling;
compared to the environmental impacts caused by actual
production.
— C4, disposal;
System boundary including provision and all transport, provision of all materials,
products and related energy and water use.
The type of EPD is according to EN 15804: "cradle to gate with
options, modules C1–C4, and module D".
Module D (Benefits and loads beyond the system boundary)
The following modules are declared: A1-A3, C, D and additional
includes:
modules: A4 + A5 + B6
— D, recycling potentials, expressed as net impacts and
Production - Module A1-A3
benefits.
The product stage includes:
Geographic Representativeness
— A1, raw material extraction, processing of secondary
Land or region, in which the declared product system is
material input (e.g. recycling processes),
manufactured, used or handled at the end of the product´s
lifespan: Germany
— A2, transport to the manufacturer,
— A3, manufacturing and assembly, processing and Comparability
mechanical treatments,including provision of all materials,
Basically, a comparison or an evaluation of EPD data is only
products and energy, as well as waste processing up to the
possible if all the data sets to be compared were created
end-of waste state.
according to EN 15804 and the building context, respectively
the product-specific characteristics of performance, are taken
Construction stage - Modules A4-A5
into account. Background database: GaBi, SP40.
The construction process stage includes:
LCA: Scenarios and additional technical information
Characteristic product properties shall be separately declared for the product and for any
Information on biogenic carbon accompanying packaging.
If the total mass of biogenic carbon containing materials is less
The biogenic carbon content quantifies the amount of biogenic than 5 % of the total mass of the product and accompanying
carbon in a construction product leaving the factory gate, and it packaging, the declaration of biogenic carbon content may be
3 Environmental-Product Declaration - dormakaba - c-lever pro
omitted. The mass of packaging containing biogenic carbon
Reference service life
shall always be declared.
Name Value Unit
Note: 1 kg of biogenic carbon is equivalent to 44/12 kg of CO2. Life Span according to the manufacturer 10 a
Operational energy use (B6) and Operational water use
Information on describing the biogenic Carbon Content at
(B7)
factory gate
The use stage is declared for 10 years.
Name Value Unit
Name Value Unit
kg
Biogenic carbon content in product 0.003024 Electricity consumption for 1 years 0,00001 kWh
C
Days per year in use 365 days
Biogenic carbon content in accompanying kg
0.08256 Stand by mode per day 23,3 h
packaging C
On mode per day 0,7 h
Stand by power 1.96E-06 W
The following technical scenario information is required for the
declared modules. On mode power 8.40E-07 W
Transport to the building site (A4) End of life (C1-C4)
Name Value Unit C1: The product dismantling from the building is
Litres of fuel 0.005925 l/100km done manually without environmental burden.
Transport distance 100 km Name Value Unit
Capacity utilisation (including empty runs) 51 % Recycling 1.8366 kg
Energy recovery 0.05733 kg
Installation into the building (A5)
Landfilling 0.057 kg
Name Value Unit
Transportation to Waste Processing Site 50 km
Waste packaging (Paper) 0.192 kg
The product is disassembled in a recycling process.
Material recycling is then assumed for the metals,
In case a reference service life according to applicable ISO
electronic and electromechanics. The plastic
standards is declared then the assumptions and in-use
components are assumed to be incinerated with
conditions underlying the determined RSL shall be declared. In
energy recovery. Minor proportions of residues arising
addition, it shall be stated that the RSL applies for the reference
from the recycling process are landfilled (1%).
conditions only.
Region for the End of Life is: Global.
The same holds for a service life declared by the manufacturer.
Reuse, recovery and/or recycling potentials (D), relevant
Corresponding information related to in-use conditions needs
scenario information
not be provided if a service life taken from the list on service life
Collection rate is 100%
by BNB is declared.
4 Environmental-Product Declaration - dormakaba - c-lever pro
LCA: Results
Disclaimer EP-freshwater: This indicator has been calculated as “kg P eq” as
required in the characterization model (EUTREND model, Struijs et al., 2009b,
as implemented in ReCiPe; http://eplca.jrc.ec.europa.eu/LCDN/developerEF.xhtml).
DESCRIPTION OF THE SYSTEM BOUNDARY (X = INCLUDED IN LCA; ND = MODULE OR INDICATOR NOT DECLARED; MNR =
MODULE NOT RELEVANT)
BENEFITS
AND LOADS
CONSTRUCTION
BEYOND
PRODUCT STAGE PROCESS USE STAGE END OF LIFE STAGE
THE SYSTEM
STAGE
BOUNDARIE
S
la ire ta m w a Ry lp p u s tro p s n a rT g n iru tc a fu n a M e h t m o rf tro p s n a rTe tis e h t o t e ta g y lb m e s s A e s U e c n a n e tn ia M ria p e R tn e m e c a lp e R tn e m h s ib ru fe R y g re n e la n o ita re p Oe s u re ta w la n o ita re p Oe s u n o itc u rts n o c -e Dn o itilo m e d tro p s n a rT g n is s e c o rp e ts a W la s o p s iD -e s u e R-y re v o c e R-g n ilc y c e Rla itn e to p
A1 A2 A3 A4 A5 B1 B2 B3 B4 B5 B6 B7 C1 C2 C3 C4 D
X X X X X MND MND MNR MNR MNR X MND X X X X X
RESULTS OF THE LCA - ENVIRONMENTAL IMPACT according to EN 15804+A2: 1 piece c-lever pro
Parameter Unit A1-A3 A4 A5 B6 C1 C2 C3 C4 D
GWP-total kg CO 2 eq 1.34E+01 1.87E-02 2.72E-01 3.76E-05 0 8.44E-03 9.66E-02 8.7E-04 -6.32E+00
GWP-fossil kg CO 2 eq 1.36E+01 1.79E-02 6.82E-03 3.74E-05 0 8.07E-03 9.66E-02 8.65E-04 -6.32E+00
GWP-biogenic kg CO 2 eq -1.63E-01 8.28E-04 2.65E-01 1.25E-07 0 3.73E-04 2.25E-06 2.95E-06 2.79E-03
GWP-luluc kg CO 2 eq 1.45E-02 4.26E-07 4.48E-06 5.43E-08 0 1.92E-07 5.46E-06 2.49E-06 -6.86E-03
ODP kg CFC11 eq 1.52E-10 1.89E-18 4.91E-17 8.24E-19 0 8.52E-19 4.87E-17 3.21E-18 -2.17E-14
AP mol H+ eq 7.86E-02 1.79E-05 7.62E-05 8.26E-08 0 8.08E-06 1.72E-05 6.2E-06 -4.4E-02
EP-freshwater kg P eq 3.73E-05 3.83E-09 9.6E-09 1E-10 0 1.73E-09 7.77E-09 1.49E-09 -1.03E-05
EP-marine kg N eq 1.09E-02 5.71E-06 2.75E-05 1.84E-08 0 2.57E-06 3.88E-06 1.6E-06 -5.73E-03
EP-terrestrial mol N eq 1.17E-01 6.34E-05 3.43E-04 1.93E-07 0 2.86E-05 7.83E-05 1.75E-05 -6.2E-02
kg NMVOC
POCP 3.28E-02 1.61E-05 7.3E-05 5.03E-08 0 7.27E-06 1.07E-05 4.83E-06 -1.84E-02
eq
ADPE kg Sb eq 4.03E-03 5.37E-10 7.75E-10 1.08E-11 0 2.42E-10 6.68E-10 7.77E-11 -2.08E-03
ADPF MJ 1.82E+02 2.54E-01 8.59E-02 6.58E-04 0 1.14E-01 4.48E-02 1.13E-02 -7.7E+01
m3 world eq
WDP 3.79E+00 3.51E-05 3.38E-02 8.16E-06 0 1.58E-05 9.88E-03 9.06E-05 -1.72E+00
deprived
GWP = Global warming potential; ODP = Depletion potential of the stratospheric ozone layer; AP = Acidification potential of land and water; EP =
Eutrophication potential; POCP = Formation potential of tropospheric ozone photochemical oxidants; ADPE = Abiotic depletion potential for non-fossil
resources; ADPF = Abiotic depletion potential for fossil resources; WDP = Water (user) deprivation potential)
RESULTS OF THE LCA - INDICATORS TO DESCRIBE RESOURCE USE according to EN 15804+A2: 1 piece c-lever pro
Parameter Unit A1-A3 A4 A5 B6 C1 C2 C3 C4 D
PERE MJ 5.02E+01 8.01E-04 2.32E+00 2.92E-04 0 3.61E-04 9.56E-02 1.49E-03 -1.47E+01
PERM MJ 2.38E+00 0 -2.3E+00 0 0 0 -8.4E-02 0 0
PERT MJ 5.26E+01 8.01E-04 1.56E-02 2.92E-04 0 3.61E-04 1.16E-02 1.49E-03 -1.47E+01
PENRE MJ 1.81E+02 2.54E-01 8.6E-02 6.58E-04 0 1.15E-01 1.49E+00 1.13E-02 -7.71E+01
PENRM MJ 1.45E+00 0 0 0 0 0 -1.45E+00 0 0
PENRT MJ 1.83E+02 2.54E-01 8.6E-02 6.58E-04 0 1.15E-01 4.48E-02 1.13E-02 -7.71E+01
SM kg 7.64E-01 0 0 0 0 0 0 0 0
RSF MJ 0 0 0 0 0 0 0 0 0
NRSF MJ 0 0 0 0 0 0 0 0 0
FW m3 1.15E-01 1.44E-06 7.95E-04 3.37E-07 0 6.47E-07 2.36E-04 2.86E-06 -6.22E-02
PERE = Use of renewable primary energy excluding renewable primary energy resources used as raw materials; PERM = Use of renewable primary
energy resources used as raw materials; PERT = Total use of renewable primary energy resources; PENRE = Use of non-renewable primary energy
excluding non-renewable primary energy resources used as raw materials; PENRM = Use of non-renewable primary energy resources used as raw
materials; PENRT = Total use of non-renewable primary energy resources; SM = Use of secondary material; RSF = Use of renewable secondary fuels;
NRSF = Use of non-renewable secondary fuels; FW = Use of net fresh water
RESULTS OF THE LCA – WASTE CATEGORIES AND OUTPUT FLOWS according to EN 15804+A2:
1 piece c-lever pro
Parameter Unit A1-A3 A4 A5 B6 C1 C2 C3 C4 D
HWD kg 1.57E-06 2.47E-11 1.27E-10 2.72E-13 0 1.11E-11 1.71E-10 1.73E-10 -1.06E-06
NHWD kg 9.31E-01 2.6E-05 8.53E-03 4.67E-07 0 1.17E-05 1E-02 5.71E-02 -1.8E-01
RWD kg 8.68E-03 2.73E-07 4.52E-06 9.99E-08 0 1.23E-07 1.66E-06 1.29E-07 -2.23E-03
CRU kg 0 0 0 0 0 0 0 0 0
MFR kg 0 0 0 0 0 0 1.86E+00 0 0
5 Environmental-Product Declaration - dormakaba - c-lever pro
MER kg 0 0 0 0 0 0 0 0 0
EEE MJ 2.14E-01 0 4.12E-01 0 0 0 0 0 0
EET MJ 3.89E-01 0 7.47E-01 0 0 0 0 0 0
HWD = Hazardous waste disposed; NHWD = Non-hazardous waste disposed; RWD = Radioactive waste disposed; CRU = Components for re-use;
MFR = Materials for recycling; MER = Materials for energy recovery; EEE = Exported electrical energy; EET = Exported thermal energy
RESULTS OF THE LCA – additional impact categories according to EN 15804+A2-optional:
1 piece c-lever pro
Parameter Unit A1-A3 A4 A5 B6 C1 C2 C3 C4 D
Disease
PM 9.04E-07 9.43E-11 4.22E-10 6.93E-13 0 4.25E-11 2.19E-10 7.68E-11 -5.54E-07
incidence
IR kBq U235 eq 8.57E-01 3.9E-05 6.99E-04 1.64E-05 0 1.76E-05 1.5E-04 1.33E-05 -2.49E-01
ETP-fw CTUe 1.19E+02 1.8E-01 4.08E-02 2.82E-04 0 8.11E-02 1.68E-02 6.48E-03 -3.36E+01
HTP-c CTUh 8.06E-07 3.39E-12 2.16E-12 7.78E-15 0 1.53E-12 1.45E-12 9.6E-13 5.51E-09
HTP-nc CTUh 5.68E-07 1.45E-10 9.35E-11 2.86E-13 0 6.53E-11 1.47E-10 1.06E-10 1.24E-06
SQP SQP 7.97E+01 6.53E-04 2.28E-02 2.1E-04 0 2.94E-04 1.34E-02 2.37E-03 -6.98E+00
PM = Potential incidence of disease due to PM emissions; IR = Potential Human exposure efficiency relative to U235; ETP-fw = Potential comparative
Toxic Unit for ecosystems; HTP-c = Potential comparative Toxic Unit for humans (cancerogenic); HTP-nc = Potential comparative Toxic Unit for humans
(not cancerogenic); SQP = Potential soil quality index
Disclaimer 1 – for the indicator IRP
This impact category deals mainly
with the eventual impact of low dose ionizing radiation on human health
of the nuclear fuel cycle. It does not consider effects due to
possible nuclear accidents, occupational exposure nor due to radioactive
waste disposal in underground facilities. Potential ionizing radiation
from the soil, from radon and from some construction materials is also
not measured by this indicator.
Disclaimer 2 – for the indicators ADPE,
ADPF, WDP, ETP-fw, HTP-c, HTP-nc, SQP
The results of this environmental
impact indicator shall be used with care as the uncertainties on these
results are high or as there is limited experience with the indicator.
References
Standards essential requirements of article 6 of Directive 2014/30/EU.
EN 301489-3 V2.2:2017-03
EN 1906:2012 Electromagnetic compatibility and Radio spectrum Matters
Building hardware - Lever handles and knob furniture - (ERM) - ElectroMagnetic Compatibility (EMC) standard for radio
Requirements and test methods; German version EN equipment and services - Part 3:
1906:2012. Specific conditions for Short-Range Devices (SRD) operating
on frequencies between 9 kHz and 246 GHz - Harmonised
EN 16867:2020 Standard covering the essential requirements ofarticle 3.1(b) of
Building hardware - Mechatronic door furniture - Requirements Directive 2014/53/EU.
and test methods; German version EN 16867:2020. EN 301489-17 V3.1.1:2017-07
EN 15804:2019+A2 ElectroMagnetic Compatibility (EMC) standard for radio
equipment and services - Part 17: Specific conditions for
EN 15804:2019+A2 (in press), Sustainability of construction Broadband Data Transmission Systems - Harmonised Standard
works — Environmental Product Declarations — Core rules for covering the essential requirements of article 3.1(b) of Directive
the product category of construction products. 2014/53/EU.
EN 300328 V2.1.1:2016-11 EN 50364:2010
Wideband transmission systems - Data transmission equipment Limitation of human exposure to electromagnetic fields from
operating in the 2,4 GHz ISM band and using wide band devices operating in the frequency range 0 Hz to 300 GHz,
modulation techniques - Harmonised Standard covering the used in Electronic Article Surveillance (EAS), Radio Frequency
essential requirements of article 3.2 of the Directive Identification (RFID) and similar applications.
2014/53/EU. EN 60529:2014-09
EN 300330 V2.1.1:2017-02 Degrees of protection provided by enclosures (IP Code, IEC
Short Range Devices (SRD) - Radio equipment in the 60529:1989 + A1:1999 + A2:2013).
frequency range 9 kHz to 25 MHz and inductive loop systems in ISO 14025:2011-10
the frequency range 9 kHz to 30 MHz - Harmonised Standard
covering the essential requirements of article 3.2 of the DIN EN ISO 14025:2011-10, Environmental labels and
Directive 2014/53/EU (Endorsement of the English version EN declarations — Type III environmental declarations —
300 330 V2.1.1 (2017-02) as German standard). Principles and procedures.
EN 301489-1 V2.2:2017-03 Radio Equipment Directive (RED)
ElectroMagnetic Compatibility (EMC) standard for radio Directive 2014/53/EU of the European Parliament and of the
equipment and services - Part 1: Common technical Council of 16 April 2014 on the harmonisation of the laws of the
requirements - Harmonised Standard covering the essential Member States relating to the making available on the market
requirements of article 3.1(b) of Directive 2014/53/EU and the of radio equipment and repealing Directive 1999/5/EC.
6 Environmental-Product Declaration - dormakaba - c-lever pro
Echterdingen
Registration, Evaluation, Authorisation and Restriction of
Chemicals (REACH) GaBi ts documentation
Regulation (EC) No 1907/2006 of the European Parliament and GaBi life cycle inventory data documentation (https://www.gabi-
of the Council on the Registration, Evaluation, Authorisation software.com/support/gabi/gabi-database-2020-lci-
and Restriction of Chemicals (REACH). documentation/).
Restriction of Hazardous Substances (RoHS)
Directive on the restriction of the use of certain hazardous LCA-tool dormakaba
substances in electrical and electronic equipment (RoHS), LCA tool, version 1.0.
Directive (EU) No 2011/65. Developed by Sphera Solutions GmbH.
Further References PCR Part A
PCR – Part A: Calculation Rules for the Life Cycle As-sessment
IBU and Requirements on the Project Re-port according to EN
Institut Bauen und Umwelt e.V.: General Programme 15804+A2:2019, Version 1.0, Institut Bauen und Umwelt e.V.,
Instructions for the Preparation of EPDs at the Institut Bauen www.ibu-epd.com.
und Umwelt e.V. Version 1., Berlin: Institut Bauen und Umwelt
e.V., 2016. www.ibu-epd.com GaBi ts software PCR Part B
Sphera Solutions GmbH PCR – Part B: Requirements on the EPD for Building Hardware
Gabi Software System and Database for Life Cycle Engineering product, version 1.2, Institut Bauen und Umwelt e.V., www.ibu-
1992-2020 Version 10.0.0.71 University of Stuttgart Leinfelden- epd.com, 2017.
7 Environmental-Product Declaration - dormakaba - c-lever pro
Publisher
Institut Bauen und Umwelt e.V. +49 (0)30 3087748- 0
Hegelplatz 1 info@ibu-epd.com
10117 Berlin www.ibu-epd.com
Germany
Programme holder
Institut Bauen und Umwelt e.V. +49 (0)30 3087748- 0
Hegelplatz 1 info@ibu-epd.com
10117 Berlin www.ibu-epd.com
Germany
Author of the Life Cycle Assessment
Sphera Solutions GmbH +49 711 341817-0
Hauptstraße 111- 113 info@sphera.com
70771 Leinfelden-Echterdingen www.sphera.com
Germany
Owner of the Declaration
dormakaba International Holding GmbH +49 2333 793-0
DORMA Platz 1 info.de@dormakaba.com
58256 Ennepetal www.dormakaba.com
Germany
8 Environmental-Product Declaration - dormakaba - c-lever pro
