ENVIRONMENTAL PRODUCT DECLARATION
as per ISO 14025 and EN 15804+A2
Owner of the Declaration Cembrit Holding A/S
Publisher Institut Bauen und Umwelt e.V. (IBU)
Programme holder Institut Bauen und Umwelt e.V. (IBU)
Declaration number EPD-CEM-20220357-CBA1-EN
Issue date 09.06.2023
Valid to 08.06.2028
Cembrit Multi Force
CEMBRIT
www.ibu-epd.com | https://epd-online.com
General Information
CEMBRIT Cembrit Multi Force
Programme holder Owner of the declaration
IBU – Institut Bauen und Umwelt e.V. Cembrit Holding A/S
Hegelplatz 1 Sohngaardsholmsvej 2
10117 Berlin 9100 Aalborg
Germany Denmark
Declaration number Declared product / declared unit
EPD-CEM-20220357-CBA1-EN 1m2 of Cembrit Multi Force fibre cement board
This declaration is based on the product category rules: Scope:
Fibre cement / Fibre concrete, 01.08.2021 This declaration including data collection, represents the production
(PCR checked and approved by the SVR) of 1 m² of Cembrit Multi Force fibre cement board on the production site
located in Lohja, Finland. Product specific data are
based on production values from the year 2019.
Issue date The owner of the declaration shall be liable for the underlying information
and evidence; the IBU shall not be liable with respect to manufacturer
09.06.2023
information, life cycle assessment data and evidences.
The EPD was created according to the specifications of EN 15804+A2. In
Valid to
the following, the standard will be simplified as EN 15804.
08.06.2028
Verification
The standard EN 15804 serves as the core PCR
Independent verification of the declaration and data according to ISO
14025:2011
internally X externally
Dipl.-Ing. Hans Peters
(Chairman of Institut Bauen und Umwelt e.V.)
Dipl.-Ing. Hans Peters Dr. Eva Schmincke,
(Managing Director Institut Bauen und Umwelt e.V.) (Independent verifier)
1 Environmental Product Declaration - CEMBRIT - Cembrit Multi Force
Product
Additional information can be found on Cembrit's website:
Product description/Product definition www.cembrit.com/downloads
Cembrit Multi Force is an indoor interior cladding panel and is
produced in both 9mm and 12mm thicknesses. Cembrit Multi Product according to the CPR, based on a hEN]: Performance
Force is easily recognized by its cement grey colour with a data of the product in accordance with the declaration of
glitter on the surface. performance with respect to its essential characteristics
It is made of cement and limestone filler, and reinforced with a according to EN 12467:2012+A2:2018 'Fibre-cement flast
specially selected fibre material. sheets. Product specification and test methods'.
Cembrit Multi Force is a versatile building board designed to be
moisture and mould resistant, impact resistant, non- Base materials/Ancillary materials
combustible, and noise reducing. The main constituents of the Cembrit Multi Force are as follows:
• Portland Cement: 45-65% (Grey)
This EPD is based on the production of 1m2 of Cembrit
• Cellulose: 5-15%
Multiforce produced in Lohja, Finland. Both the 9mm board and
• Inert filler: 10-25%
12 mm Multiforce are produced at this production site.
• Light weight filler: 10-20%
• Mica: 10-20%
Cembrit Multiforce is sold throughout various countries in
• Pigments: 5%
Europe under the names: Luja A, Cembrit Sauna, Internit LW.
There are no substances of very high concern (SVHC) present
More information can be found in the Declaration of
in the construction of the product.
Performance found on Cembrit's home website in the
downloads section: https://www.cembrit.com/downloads? Reference service life
type=dop For the placing on the market of the product in the Cembrit Multi Force is introduced quite recently on the market.
European Union/European Free Trade Association (EU/EFTA) There are no substantiated data on the reference service life
(with the exception of Switzerland) Regulation (EU) No. (RSL). However, it is estimated that the RSL of Cembrit Multi
305/2011 (CPR) applies. The product needs a declaration of Force is 50 years or higher. This is in accordance with the table
performance taking into consideration EN12467:2012+A1:2016/ published by the Bundesinstitut für Bau-, Stadt- und
and the CE marking. Raumforschung (BBSR) (code 335.511).
Disclaimer: The BBSR estimation of the RSL of fibre cement
Application
products relates to facade and roofing products. Nevertheless,
Walls, both shaft- and partition walls where fire protection,
Cembrit Multi Force (indoor board) is expected to have an RSL
sound insulation and durability are needed, are natural places
of 50 years or higher, as it sustains lower impacts relating to
for Cembrit Multi Force. It can also be used in suspended
natural weathering.
ceilings, and balconies. The Outdoor environment is not a
problem as long as the product does not freeze when soaking
wet.
Technical Data
The following technical data are to be mentioned:
Constructional data
Name Value Unit
Thermal conductivity 0.23 W/mK
Water vapour diffusion resistance factor acc. to
30.5 -
DIN V 4108-4, EN ISO 12572
Swelling (air-dry to water-saturated) 2.2 mm/m
Gross density (average) 1158 kg/m3
Tensile strength 5 N/mm2
Flexural strength 10 N/mm2
Modulus of elasticity 4000 N/mm2
LCA: Calculation rules
Name Value Unit
Declared Unit
Declared unit 1 m^2
In this EPD the declared unit is defined as the production of
Gross density 1158 kg/m^3
1m2 "Cembrit Multi Force" fibre cement sheet, with ANexpected
lifetime of 50 years or higher, and its related impacts over the Area weight 10.42 kg/m^2
'cradle to grave' life-cycle modules. Data is gathered for the production process at Cembrit's factory
site in Finland (Lohja), for the year 2019.
The LCA data is based on the production of Multiforce with a
thickness of 9mm. Therefore, a conversion factor of 1,33 is System boundary
needed to calculate results for a Multiforce of 12mm thickness The modules considered in this EPD follows a cradle to gate
and is valid for all the indicators. The reference year of the LCA with options: A1-A5, C1-C4, D.
data is 2019. A1 - The system boundaries includes the provision and
processing of raw materials. These include in particular cement,
Declared unit and mass reference
plastic fibres, pulp and packaging materials.
2 Environmental Product Declaration - CEMBRIT - Cembrit Multi Force
C3 - The fibre cement boards are sent to landfill and therefore
A2 - The transports to the manufacturer were specifically there are no environmental impacts associated with waste
collected for all starting materials. processing of materials flows intended for reuse, recycling or
energy recovery.
A3 - The production includes also all in-plant energy
consumption (gas + electricity), as well as water used in the C4 - Environmental impacts associated with the processes at
production process, and production waste. the landfill.
A4 - The transport, part of the construction process, is an D - The fibre cement boards are sent to landfill after use. The
average of the total distance of all products delivered to the product has therefore no impact during this stage and no
point of installation. This is calculated to be 2064 km. associated environmental impacts. The boards are expected
to be reusable over time, but this is not included in this
A5 - All environmental impacts associated with the disposal of assessment. Recycling credit for the product along with
packaging handled at the construction site are accounted for. It incineration credit for the packaging material have been
is assumed incinerated at an incineration plant. Disposal of considered.
product waste is assumed to be landfilled. Furthermore,
environmental impacts associated Geographic Representativeness
with trucks and fuel for the construction installation are Land or region, in which the declared product system is
included. manufactured, used or handled at the end of the product´s
lifespan: Europe
C1 - Accounts for the environmental impacts associated with
dismantling and demolition of the fibre cement boards. Fuel
Comparability
used for demolition equipment and transport on-site vehicles.
Basically, a comparison or an evaluation of EPD data is only
possible if all the data sets to be compared were created
C2 - Transportation of the discarded products from the
according to EN 15804 and the building context, respectively
construction site to a landfilling site. The transport is estimated
the product-specific characteristics of performance, are taken
to be 100 km in an average truck.
into account. The database used is DB CUP 2021.1
LCA: Scenarios and additional technical information
installation point. Cembrit's warehouses for which the distance
Characteristic product properties of biogenic carbon has been calculated are located in Denmark, Sweden, Norway,
The biogenic carbon containing material (cellulose) in Cembrit Netherlands, Belgium, Ireland and the United Kingdom.
Multi Force is >5% of its total mass of the product and is
therefore required to be listed separately. The following table
Name Value Unit
shows the biogenic carbon content in the product and
Transport distance 2064 km
accompanying packaging:
Gross density of products transported 1158 kg/m3
Information on describing the biogenic Carbon Content at
factury gate
Installation into the building (A5)
Name ValueUnit Installation of the boards is carried out by use of an automatic
kg screwdriver. It is estimated that 12 screws are used for the
Biogenic carbon content in product 0.003
C installation of the declared unit of Cembrit Multi Force.
Biogenic carbon content in accompanying kg
0.004
packaging C Furthermore, packaging waste generated in the installation of
the boards is depicted in this module.
Name Value Unit
The following technical scenario information is required for the
declared modules and optional for non-declared modules. Plastic waste 0.008 kg
Modules for which no information is declared can be deleted; Pallets 0.007 kg
additional information can also be listed if necessary. Screws 12 pcs
The following technical information is a basis for the declared
In case a reference service life according to applicable ISO
modules or can be used for developing specific scenarios in the
standards is declared then the assumptions and in-use
context of a building assessment if modules are not declared
conditions underlying the determined RSL shall be declared. In
(MND).
addition, it shall be stated that the RSL applies to the reference
A5 is not declared including the disposal of the packaging conditions only.
material on the construction site, the amounts of packaging
The same holds for a service life declared by the manufacturer.
materials included in the LCA calculations must be declared as
Corresponding information related to in-use conditions needs
technical scenario information for Module A5.
not be provided if a service life taken from the list of service life
by BNB is declared.
Transport to the building site (A4)
Reference service life
Estimating the transport to each individual construction site is
rather complex. However, an educated estimate is made for the
distance to the installation point by averaging the total distance
of all products delivered to Cembrit's warehouses and adding
100 km, representing the distance from warehouse to
3 Environmental Product Declaration - CEMBRIT - Cembrit Multi Force
Name Value Unit processing of material flows intended for reuse, recycling or
energy recovery. Reuse and recycling of the boards is possible;
Reference service life (according to ISO
- a however, such a system is not extensively considered yet.
15686-1, -2, -7 and -8)
Transportation
Equal or more
Life Span (according to BBSR) a of the discarded products from the construction site to a
than 50
landfilling site is assumed to be ~100 km in an average truck.
Life Span according to the manufacturer - a
Name Value Unit
End of life (C1-C4) and D (reuse) Energy recovery (packaging) 0.0154 kg
Currently, the fibre cement boards are sent to landfill and no Landfilling 10.42 kg
environmental impacts are therefore associated with waste
4 Environmental Product Declaration - CEMBRIT - Cembrit Multi Force
LCA: Results
The following tables show the results of life-cycle assessment indicators, resource use and waste related to 1m2 of Cembrit Multi Force
fibre cement boards.The data is representative of the products of Cembrit Holding A/S.
DESCRIPTION OF THE SYSTEM BOUNDARY (X = INCLUDED IN LCA; ND = MODULE OR INDICATOR NOT DECLARED; MNR =
MODULE NOT RELEVANT)
Benefits and
Construction loads beyond
Product stage Use stage End-of-life stage
process stage the system
boundaries
la ire ta m w a Ry lp p u s tro p s n a rT g n iru tc a fu n a M e h t m o rf tro p s n a rTe tis e h t o t e ta g y lb m e s s A e s U e c n a n e tn ia M ria p e R tn e m e c a lp e R tn e m h s ib ru fe R y g re n e la n o ita re p Oe s u re ta w la n o ita re p Oe s u n o itc u rts n o c -e Dn o itilo m e d tro p s n a rT g n is s e c o rp e ts a W la s o p s iD -e s u e R-y re v o c e R-g n ilc y c e Rla itn e to p
A1 A2 A3 A4 A5 B1 B2 B3 B4 B5 B6 B7 C1 C2 C3 C4 D
X X X X X MND MND MNR MNR MNR MND MND X X X X X
RESULTS OF THE LCA - ENVIRONMENTAL IMPACT according to EN 15804+A2: 1 m2 Cembrit Multi Force
Parameter Unit A1 A2 A3 A4 A5 C1 C2 C3 C4 D
GWP-total kg CO 2 eq 4.94E+00 4.12E-01 2.48E+00 1.32E+00 7.62E-01 4.77E-04 1.32E+00 -6.57E-01 1.06E+00 -4E-03
GWP-fossil kg CO 2 eq 4.94E+00 3.95E-01 2.48E+00 1.27E+00 7.48E-01 4.72E-04 1.27E+00 2.46E-01 1.61E-01 -4E-03
GWP-
biogenic kg CO 2 eq 5E-03 1.7E-02 -5E-03 5.8E-02 1.4E-02 4.02E-06 5.8E-02 -9.03E-01 8.99E-01 -1.97E-05
GWP-luluc kg CO 2 eq 1E-03 9.34E-06 1.53E-04 3E-05 5.27E-04 6.69E-07 3E-05 6.28E-04 4.72E-04 -2.67E-06
ODP kg CFC11 eq 8.55E-15 4.52E-17 4.53E-15 1.45E-16 5.18E-15 1.13E-17 1.45E-16 6.03E-12 6.25E-16 -4.4E-17
AP mol H+ eq 1.5E-02 9.15E-04 2E-03 1E-03 2E-03 9.83E-07 1E-03 1E-03 1E-03 -5.16E-06
EP-
kg P eq 1.61E-06 8.37E-08 1.37E-06 2.69E-07 1.38E-06 1.27E-09 2.69E-07 1.04E-05 2.7E-07 -5.05E-09
freshwater
EP-marine kg N eq 4E-03 4.05E-04 8.25E-04 3.29E-04 4E-04 2.34E-07 3.29E-04 5.9E-04 2.97E-04 -1.49E-06
EP-terrestrial mol N eq 4.6E-02 4E-03 9E-03 4E-03 4E-03 2.45E-06 4E-03 6E-03 3E-03 -1.6E-05
kg NMVOC
POCP 1.2E-02 1E-03 2E-03 9.95E-04 1E-03 6.34E-07 9.95E-04 2E-03 9.01E-04 -4.18E-06
eq
ADPE kg Sb eq 1.75E-07 1.38E-08 1.4E-07 4.42E-08 3.78E-05 1.39E-10 4.42E-08 9.48E-08 1.52E-08 -6.51E-10
ADPF MJ 2.91E+01 5.58E+00 3.65E+01 1.79E+01 7.58E+00 8E-03 1.79E+01 3.42E+00 2.13E+00 -7.1E-02
m3 world eq
WDP 1.47E-01 6.53E-04 1.58E-01 2E-03 1.7E-02 7.58E-05 2E-03 4.8E-02 1.7E-02 -2.95E-04
deprived
GWP = Global warming potential; ODP = Depletion potential of the stratospheric ozone layer; AP = Acidification potential of land and water; EP =
Eutrophication potential; POCP = Formation potential of tropospheric ozone photochemical oxidants; ADPE = Abiotic depletion potential for non-fossil
resources; ADPF = Abiotic depletion potential for fossil resources; WDP = Water (user) deprivation potential)
RESULTS OF THE LCA - INDICATORS TO DESCRIBE RESOURCE USE according to EN 15804+A2: 1 m2 Cembrit Multi Force
Parameter Unit A1 A2 A3 A4 A5 C1 C2 C3 C4 D
PERE MJ -4.43E+00 1.8E-02 1.12E+00 5.9E-02 1.7E+00 4E-03 5.9E-02 1.81E+01 7.78E+00 -1.5E-02
PERM MJ 7.49E+00 0 1.4E-01 0 -1.4E-01 0 0 0 -7.49E+00 0
PERT MJ 3.06E+00 1.8E-02 1.26E+00 5.9E-02 1.56E+00 4E-03 5.9E-02 1.81E+01 2.87E-01 -1.5E-02
PENRE MJ 2.91E+01 5.58E+00 3.62E+01 1.8E+01 7.96E+00 8E-03 1.8E+01 3.42E+00 2.13E+00 -7.1E-02
PENRM MJ 0 0 3.4E-01 0 -3.4E-01 0 0 0 0 0
PENRT MJ 2.91E+01 5.58E+00 3.65E+01 1.8E+01 7.62E+00 8E-03 1.8E+01 3.42E+00 2.13E+00 -7.1E-02
SM kg 7E-01 0 0 0 0 0 0 0 0 0
RSF MJ 0 0 0 0 0 0 0 0 0 0
NRSF MJ 0 0 0 0 0 0 0 0 0 0
FW m3 5E-03 2.95E-05 8E-03 9.5E-05 2E-03 3.77E-06 9.5E-05 2E-03 5.26E-04 -1.48E-05
PERE = Use of renewable primary energy excluding renewable primary energy resources used as raw materials; PERM = Use of renewable primary
energy resources used as raw materials; PERT = Total use of renewable primary energy resources; PENRE = Use of non-renewable primary energy
excluding non-renewable primary energy resources used as raw materials; PENRM = Use of non-renewable primary energy resources used as raw
materials; PENRT = Total use of non-renewable primary energy resources; SM = Use of secondary material; RSF = Use of renewable secondary fuels;
NRSF = Use of non-renewable secondary fuels; FW = Use of net fresh water
RESULTS OF THE LCA – WASTE CATEGORIES AND OUTPUT FLOWS according to EN 15804+A2:
1 m2 Cembrit Multi Force
Parameter Unit A1 A2 A3 A4 A5 C1 C2 C3 C4 D
HWD kg 1.97E-09 3.84E-11 7.09E-09 1.23E-10 9.76E-10 2.22E-12 1.23E-10 1.35E-07 2.27E-10 -1.57E-11
NHWD kg 1.9E-02 5.59E-04 3.14E-01 2E-03 1.2E-02 5.96E-06 2E-03 2E-02 1.06E+01 -3.18E-05
RWD kg 9.86E-04 5.98E-06 5E-03 1.92E-05 2.97E-04 1.25E-06 1.92E-05 1.72E-04 2.24E-05 -4.87E-06
CRU kg 0 0 0 0 0 0 0 0 0 0
MFR kg 0 0 0 0 0 0 0 0 0 0
MER kg 0 0 0 0 0 0 0 0 0 0
5 Environmental Product Declaration - CEMBRIT - Cembrit Multi Force
EEE MJ 0 0 0 0 7.33E-06 0 0 0 0 0
EET MJ 0 0 0 0 7.33E-06 0 0 0 0 0
HWD = Hazardous waste disposed; NHWD = Non-hazardous waste disposed; RWD = Radioactive waste disposed; CRU = Components for re-use;
MFR = Materials for recycling; MER = Materials for energy recovery; EEE = Exported electrical energy; EET = Exported thermal energy
RESULTS OF THE LCA – additional impact categories according to EN 15804+A2-optional:
1 m2 Cembrit Multi Force
Parameter Unit A1 A2 A3 A4 A5 C1 C2 C3 C4 D
Disease
PM 2.11E-07 1.22E-08 2.08E-08 5.79E-09 2.13E-08 8.29E-12 5.79E-09 1.86E-08 1.42E-08 -4.45E-11
incidence
IR kBq U235 eq 1.52E-01 8.47E-04 4.84E-01 3E-03 3.7E-02 2.05E-04 3E-03 2.8E-02 2E-03 -7.98E-04
ETP-fw CTUe 1.58E+01 4.04E+00 8.58E+00 1.3E+01 2.08E+00 4E-03 1.3E+01 1.58E+00 1.22E+00 -1.4E-02
HTP-c CTUh 6.52E-10 7.52E-11 2.09E-10 2.42E-10 7.51E-10 1E-13 2.42E-10 7.51E-11 1.79E-10 -6.63E-13
HTP-nc CTUh 6.21E-08 3.16E-09 1.8E-08 1.01E-08 8.75E-09 3.78E-12 1.01E-08 4.05E-09 1.98E-08 -2.63E-11
SQP SQP 2.33E+00 1.4E-02 3.04E+00 4.6E-02 1.27E+00 3E-03 4.6E-02 1.17E+02 4.31E-01 -1E-02
PM = Potential incidence of disease due to PM emissions; IR = Potential Human exposure efficiency relative to U235; ETP-fw = Potential comparative
Toxic Unit for ecosystems; HTP-c = Potential comparative Toxic Unit for humans (cancerogenic); HTP-nc = Potential comparative Toxic Unit for humans
(not cancerogenic); SQP = Potential soil quality index
Disclaimer 1 – for the indicator “Potential Human exposure efficiency relative to U235”. This impact category deals mainly with the
eventual impact of low dose ionizing radiation on human health of the nuclear fuel cycle. It does not consider effects due to possible
nuclear accidents, occupational exposure nor due to radioactive waste disposal in underground facilities. Potential ionizing radiation
from the soil, from radon and from some construction materials is also not measured by this indicator.
Disclaimer 2 – for the indicators “abiotic depletion potential for non-fossil resources”, “abiotic depletion potential for fossil resources”,
“water (user) deprivation potential, deprivation-weighted water consumption”, “potential comparative toxic unit for ecosystems”,
“potential comparative toxic unit for humans – cancerogenic”, “Potential comparative toxic unit for humans - not cancerogenic”,
“potential soil quality index”. The results of this environmental impact indicator shall be used with care as the uncertainties on these
results are high or as there is limited experienced with the indicator.
References
Standards CUP Version: 2021.1
EN 15804 University of Stuttgart
EN 15804:2012+A1:2013, Sustainability of Leinfelden Echterdingen
construction works — Environmental Product
Declarations — Core rules for the product category of GaBi documentation
construction products. GaBi life cycle inventory data documentation
(https://www.gabisoftware.com/support/gabi/gabidatabase2020lcidocumentation/)
EN 15804
EN 15804:2012+A2:2019+AC:2021, Sustainability of PCR Part A
construction works — Environmental Product Calculation Rules for the Life Cycle Assessment and
Declarations — Core rules for the product category of Requirements on the
construction products. Project Report,Berlin: Institut Bauen und Umwelt e.V., www.ibu-
epd.com,
ISO 14025 Version 2.2, 2022
EN ISO 14025:2011, Environmental labels and
declarations — Type III environmental declarations — PCR Part B
Principles and procedures. Requirements of the EPD for Fibre Cement/Fibre Concrete,
version 1.7,
EN12467 Institut Bauen und Umwelt e.V., www.bau-umwelt.com, 2019
EN12467:2012+A2:2018, Fibre-cement flat sheets — Product
specifications and test methods" IBU 2021
Institut Bauen und Umwelt e.V.: General Instructions for the
Further References EPD programme of Institut Bauen und Umwelt e.V., Version
2.0, Berlin: Institut Bauen und Umwelt e.V., 2021 www.ibu-
BBSR epd.com
Bundesinstitut für Bau-, Stadt- und Raumforschung
(BBSR): Nutzungsdauer von Bauteilen für Cembrit A/S
Lebenszyklusanalyse nach Bewertungssystem Cembrit A/S: Information on technical data and downloads.
Nachhaltiges Bauen (BNB), 2011 www.Cembrit.com/downloads
The literature referred to in the Environmental Product
GaBi software Declaration must be listed in full.Standards already fully quoted
Sphera Solutions GmbH in the EPD do not need to be listed here again.
GaBi Software System and Database for Life Cycle The current version of PCR Part A and PCR Part B of the PCR
Engineering document on which they are based must be referenced.
6 Environmental Product Declaration - CEMBRIT - Cembrit Multi Force
Publisher
Institut Bauen und Umwelt e.V. +49 (0)30 3087748- 0
Hegelplatz 1 info@ibu-epd.com
10117 Berlin www.ibu-epd.com
Germany
Programme holder
Institut Bauen und Umwelt e.V. +49 (0)30 3087748- 0
Hegelplatz 1 info@ibu-epd.com
10117 Berlin www.ibu-epd.com
Germany
Author of the Life Cycle Assessment
Sphera Solutions GmbH +49 711 341817-0
Hauptstraße 111- 113 info@sphera.com
70771 Leinfelden-Echterdingen www.sphera.com
Germany
Owner of the Declaration
Cembrit Holding A/S +45 99 37 22 22
Sohngaardsholmsvej 2 info@cembrit.com
9100 Aalborg www.cembrit.com
Denmark
7 Environmental Product Declaration - CEMBRIT - Cembrit Multi Force
