ENVIRONMENTAL PRODUCT DECLARATION
as per ISO 14025 and EN 15804+A2
Owner of the Declaration Etex Building Performance International
Programme holder Institut Bauen und Umwelt e.V. (IBU)
Publisher Institut Bauen und Umwelt e.V. (IBU)
Declaration number EPD-ETE-20220212-CCA1-EN
Issue date 24.10.2022
Valid to 23.10.2027
Cementex / Cementex Extreme
Siniat
www.ibu-epd.com | https://epd-online.com
Umwelt Produktdeklaration Name des Herstellers – Name des Produkts
General Information
Etex Building Performance International Cementex / Cementex Extreme
Programme holder Owner of the declaration
IBU – Institut Bauen und Umwelt e.V. Etex Building Performance International
Hegelplatz 1 500 Rue Marcel Demonque
10117 Berlin F-84915 Avignon
Germany France
Declaration number Declared product / declared unit
EPD-ETE-20220212-CCA1-EN The functional unit is 1 m2 of Cementex / Cementex
Extreme of 10mm thickness.
The EPD also has an annexe which describes the
impacts for 1m2 Cementex / Cementex Extreme for the
other existing thicknesses (6 mm, 8 mm, 12 mm).
This declaration is based on the product Scope:
category rules: The life cycle assessment is based on the production
Fibre cement / Fibre concrete, 01.2019 data of Cementex / Cementex Extreme of the year
(PCR checked and approved by the SVR) 2019 at the two Etex production sites in Gresik and
Karawang, both located in Indonesia. The average of
the data collected from both plants has been used in
Issue date
this LCA study.
24.10.2022
The owner of the declaration shall be liable for the
Valid to
underlying information and evidence; the IBU shall not
23.10.2027
be liable with respect to manufacturer information, life
cycle assessment data and evidences.
The EPD was created according to the specifications
of EN 15804+A2. In the following, the standard will be
simplified as EN 15804.
Verification
The standard EN 15804 serves as the core PCR
Independent verification of the declaration and data
according to ISO 14025:2011
Dipl. Ing. Hans Peters internally x externally
(chairman of Institut Bauen und Umwelt e.V.)
Dr. Alexander Röder Vito D'Incognito
(Managing Director Institut Bauen und Umwelt e.V.)) (Independent verifier)
Product
Product description/Product definition  The product needs a declaration of
Cementex and Cementex Extreme are cellulose performance taking into consideration EN
reinforced fibre cement boards. The main difference
12467:2013+A2:2018, Fibre cement flat
between the products is that Cementex Extreme has
sheets and the CE-marking.
an additional hydrophobic layer.
 For the application and use the respective
Cementex / Cementex Extreme boards are highly national provisions apply.
durable and suitable for external and internal
applications. The boards are manufactured using
Application
the Hatschek technology and then autoclaved, which
The Cementex / Cementex Extreme boards are
ensures optimal dimensional stability and mechanical
suitable for internal and external applications.
resistance. The boards are available with squared
edges.
 Inner wall: non-load-bearing partition wall,
retaining wall, timber frame wall, steel frame
For the placing on the market of the product in the
European Union/European Free Trade Association wall.
(EU/EFTA) (with the exception of Switzerland)  Interior floor: finishing backer and loadbearing
Regulation (EU) No. 305/2011 (CPR) applies. plate on load-bearing floors and floating floors
2 Environmental Product Declaration Etex – Cementex/Cementex Extreme
 Interior ceiling: suspended ceilings, pool
ceilings
Technical Data
 Outdoor: wall and ceiling cladding in the not
The safety of a building is directly linked to the quality
directly exposed outdoor area.
of the materials employed in its construction. The use
of standardized materials and proper handling
Manufacturing Process procedures is one of the ways construction industries
Cementex fibre cement boards are manufactured ensure a building’s safety.
largely in accordance with an automated winding
process, the Hatschek process: the raw materials are Etex on-site laboratories perform chemical and
mixed with water to prepare a homogenous mixture. mechanical tests guaranteeing compliance of the final
Rotating screen cylinders are immersed in this fibre products to technical standard requirements. Technical
cement pulp which drains internally. The screen product specification is set by European standard EN
surface is covered in a thin film of fibre cement which 12467:2013 + A2:2018 ‘Fibre-cement flat sheets’.
is transferred onto an infinite conveyor belt from where
it is conveyed to a format roller or forming drum which Constructional data
is gradually covered in an increasingly thicker layer of Name Value Unit
fibre cement. Once the requisite material thickness is Thermal conductivity ISO 13787 25 W/(mK)
achieved, the still moist and malleable fibre cement Sound absorption coefficient NA %
layer (fibre cement fleece) is separated and removed Gross density EN 12467 1200 kg/m3
from the forming drum. The fibre cement fleece is cut Compressive strength - N/mm2
to size. Leftovers are returned to the production Flexural strength EN 12467 7 N/mm2
process preventing any waste from being incurred. The Modulus of elasticity 7000 N/mm2
sheets are then laid on templates and steam-hardened Moisture content at 23 °C, 80%
0.4 M.-%
in an autoclave. The Cementex boards are then humidity EN 12467
calibrated, sanded and for the Cementex Extreme Passed
boards, a hydrophobic layer is applied at both sides. Soak dry test EN 12467 (50 Cycles)
Strength classification EN 12467 Class 2
The quality management system of the production
Impermeability test EN 12467 Passed
facilities is certified according to ISO 9001;2015.
Fire reaction classification EN
A1
13501-1
Passed
Installation
Freeze-Thaw EN 12467 (100 10-6K-1
The Cementex / Cementex Extreme boards are mainly
Cycles)
fixed with screws on a metal or wooden substructure.
Warm water test EN 12467 Passed
The joints are treated with a jointing compound, a
Durability EN 12467 Category A
reinforcement tape is used over the edges and the
boards are finished with a finishing compound.
Performance data of the product in accordance with
Environment and health during manufacturing
the declaration of performance with respect to its
Environmental, occupational health and safety
essential characteristics according to
management system at the Cementex production
EN 12467:2013+A2:2018, Fibre cement flat sheets.
plants are in accordance with the following standards:
ISO 14001;2015
Base materials/Ancillary materials
ISO 45001;2018
Main raw materials used (in weight percentages):
Portland Cement - 25-45 %
Condition of use
Sand M32 - 35-50 %
Maintenance requirement will depend on the specific
Cellulose - <10 %
design and application. Usually Cementex / Cementex
others - <10 %
Extreme won’t change the composition of the materials
and thus no maintenance is needed.
This product/article/at least one partial article contains
substances listed in the candidate list (date:
Environment and health during use
24.10.2022) exceeding 0.1 percentage by mass: no.
When the boards are used as designed, the current
state of knowledge indicates that there is no risk
Reference service life
involved for the environment or health.
Cementex is a rather new product on the market
(produced since 2017), and there is not yet extensive
Water
evidence regarding its reference service life. However
All ingredients are firmly bound in the matrix. The
based on the internal experience with other fibre
boards are insensitive to moisture and no ingredients
cement products in various applications it is assumed
which could be hazardous to water are expected to be
that upon condition that the product is used in
washed out in the event of extraordinary effects by
accordance with the recommended installation
water.
guidelines, it is feasible to assume that this product
lasts for 60 years unless it is used in aggressive
Mechanical destruction
environments or fully exposed applications.
In case of mechanical destruction, no risks are
expected to occur in terms of environment and human
health.
3 Environmental Product Declaration Etex – Cementex/Cementex Extreme
LCA: Calculation rules
Declared Unit manufacturing site (A2), production of final
The functional unit is 1 m2 of Cementex / product (A3);
Cementex Extreme of 10 mm thickness.
 Construction process stage: transport to
construction site (A4), construction/installation
Name Value Unit
process (A5);
Declared unit 1 m^2
Area density with 10 mm thickness 14.6 kg/m^2  Use stage: use (B1), maintenance (B2),
repair (B3), replacements (B4), refurbishment
The data provided in the EPD, relate to the data of (B5), operational energy use (B6), operational
Cementex Extreme, which is considered to be water use (B7);
representative of Cementex and it represents the
 End-of-life stage: deconstruction/demolition
“worst case scenario”. Also, the data are the average
(C1), transport to end-of-life treatment (C2),
derived from the two production sites in Gresik and
Karawang in Indonesia. Hence a variability study was waste processing (C3) and final disposal (C4)
conducted whose results displayed that there is little to  Benefits and loads beyond the system
no difference between the results based on average boundaries: reuse, recovery, recycling
data and the data specific to the production sites. potential (D)
System boundary
This study takes into account the mandatory life cycle Comparability
stages of the EN15804+A2 for a cradle-to-grave LCA Basically, a comparison or an evaluation of EPD data
study, being modules A1, A2, A3, A4, A5, B1, B2, B3, is only possible if all the data sets to be compared
B4, B5, B6, B7, C1, C2, C3, C4 and D. were created according to EN 15804 and the building
context, respectively the product-specific
Life cycle stages: characteristics of performance, are taken into account.
 Product stage: production of raw materials
(A1), transport of raw materials to
LCA: Scenarios and additional technical information
Characteristic product properties Transport Distance (merchant to
Information on biogenic Carbon installation) Truck 3.5 – 7.5 t, 35 km
The biogenic carbon content quantifies the amount of Euro5
biogenic carbon in a construction product leaving the
factory gate. Installation into the building (A5)
Name Value Unit
There is biogenic carbon content in the product due to Auxiliary Steel screws 0.03 kg
the use of cellulose. The uptake of biogenic CO 2 within Water consumption Tap water 0.00041 m3
the pallets and the carton is reported in module A3 and Electricity consumption Electricity,
0.03617 kWh
the release in module A5. The table below shows the low voltage
biogenic carbon content per functional unit. Joint mesh tape 0.000858 kg
Primer 0.1040 kg
Information on describing the biogenic Carbon
Finisher 0.220 kg
Content at factory gate
Installation losses 3 %
Name Value Unit
Biogenic Carbon Content in
0.435 kg C
product
Use or application of the installed product (B1)
Biogenic Carbon Content in
0.189 kg C The Cementex / Cementex Extreme boards are
accompanying packaging
permanently installed in the building and generally do
not require any repair, maintenance or replacement.
The only impact during the use phase is that of
carbonation, where some CO is adsorbed from the
2
atmosphere over the life of the board. Depending on
Transport to the building site (A4)
the application where the boards are used, the degree
Name Value Unit
of carbonation will vary.
Transport Distance (factory to
merchant) Transoceanic freight 19988 km
The carbonation was calculated to be as follows for the
ship
various use scenarios and reported in the B1 module
Transport Distance (factory to
656 km as shown below,
merchant) Truck 16 – 32 t, Euro5
Transport Distance (factory to
66 km
merchant) Truck 16 – 32 t, Euro3  B1/1 - Outdoor sheltered from rain : -1.768 kg
Transport distance (merchant to CO eq / 1 m²10 mm.
35 km 2
installation) Truck 16 – 32 t, Euro5
4 Environmental Product Declaration Etex – Cementex/Cementex Extreme
 B1/2 - Indoor without or with “open” cover
such as a paint : -0.943 kg CO eq / 1 m²10
2
mm.
 B1/3 - Indoor under “closed” cover such as a
tile : 0 kg CO eq / 1 m²10 mm.
2
Name Value Unit
.
Reference service life
The RSL of Cementex / Cementex Extreme is
estimated at 60 years unless it is used in aggressive
environments or fully exposed applications
Name Value Unit
Life Span according to the
60 a
manufacturer
Outdoor environment, (for outdoor
applications), e.g. weathering,
pollutants, UV and wind exposure, 60 -
building orientation, shading,
temperature
Indoor environment (for indoor
applications), e.g. temperature, 60 -
moisture, chemical exposure
End of life (C1-C4)
A conservative approach was used in this study.
Although after end-of-life, scenarios where the boards
are re-used or recycled are realistic, a scenario with
100% landfill was used.
Name Value Unit
Collected separately waste type - kg
Collected as mixed construction
- kg
waste
Reuse - kg
Recycling Steel Screws 0.0285 kg
Energy recovery Steel Screws 0.0006789 kg
Landfilling Steel screws 0.0008211 kg
Landfilling Fibre cement board 14.83 kg
Reuse, recovery and/or recycling potentials (D),
relevant scenario information
In module D, the benefits and loads beyond the system
boundaries are quantified. For recycling, it concerns
both loads of the recycling processes and the benefits
of the avoided virgin materials, when the recycled
components are used for other purposes. In case of
incineration, it concerns the benefits from the avoided
production of energy grace to energy recovery.
Name Value Unit
5 Environmental Product Declaration Etex – Cementex/Cementex Extreme
LCA: Results
The following tables describe the environmental performance of the 1 m2 Cementex / Cementex Extreme of 10
mm thickness.
DESCRIPTION OF THE SYSTEM BOUNDARY (X = INCLUDED IN LCA; ND = MODULE OR INDICATOR NOT
DECLARED; MNR = MODULE NOT RELEVANT)
BENEFITS AND
CONSTRUCTI LOADS
PRODUCT STAGE ON PROCESS USE STAGE END OF LIFE STAGE BEYOND THE
STAGE SYSTEM
BOUNDARIES
6 Environmental Product Declaration Etex – Cementex/Cementex Extreme
lairetam
waR
ylppus tropsnarT
gnirutcafunaM
eht
morf
tropsnarT
etis
eht
ot
etag
ylbmessA esU
ecnanetniaM
riapeR
tnemecalpeR tnemhsibrufeR
ygrene
lanoitarepO esu
retaw
lanoitarepO esu
noitcurtsnoc-eD
noitilomed tropsnarT
gnissecorp
etsaW
lasopsiD -esueR -yrevoceR -gnilcyceR laitnetop
A1 A2 A3 A4 A5 B1 B2 B3 B4 B5 B6 B7 C1 C2 C3 C4 D
X X X X X X X X X X X X X X X X X
RESULTS OF THE LCA - ENVIRONMENTAL IMPACT according to EN 15804+A2: 1 m2 Cementex /
Cementex Extreme (10 mm)
Core Indicator Unit A1 A2 A3 A4 A5 B1/1 B1/2 B1/3 B2 B3 B4 B5 B6 B7 C1 C2 C3 C4 D
- - -
3.60E7.94E3.18E4.85E1.67E 0.00E0.00E0.00E0.00E0.00E0.00E0.00E8.87E1.27E6.29E1.73E
GWP-total [kg CO2-Eq.]
+0 -1 +0 +0 +0
1.77E9.43E
+0 +0 +0 +0 +0 +0 +0 -3 -1 -5 +0
1.38E
+0 -1 -1
-
5.40E7.93E3.67E4.84E9.64E0.00E0.00E0.00E0.00E0.00E0.00E0.00E0.00E0.00E8.79E1.27E6.18E1.00E
GWP-fossil [kg CO2-Eq.]
+0 -1 +0 +0 -1 +0 +0 +0 +0 +0 +0 +0 +0 +0 -3 -1 -5 -1
1.37E
-1
- - -
3.52E 1.60E7.07E0.00E0.00E0.00E0.00E0.00E0.00E0.00E0.00E0.00E6.15E5.20E1.02E1.63E
GWP-biogenic [kg CO2-Eq.] 1.80E
-4
4.93E
-3 -1 +0 +0 +0 +0 +0 +0 +0 +0 +0 -5 -5 -6 +0
1.52E
+0 -1 -4
-
2.37E4.76E7.36E2.69E7.87E0.00E0.00E0.00E0.00E0.00E0.00E0.00E0.00E0.00E2.05E4.45E7.38E5.12E
GWP-luluc [kg CO2-Eq.]
-3 -4 -3 -3 -4 +0 +0 +0 +0 +0 +0 +0 +0 +0 -5 -5 -8 -5
2.44E
-4
-
2.45E1.68E2.11E1.02E9.82E0.00E0.00E0.00E0.00E0.00E0.00E0.00E0.00E0.00E7.40E2.90E2.50E3.32E
ODP [kg CFC11-Eq.] 1.37E
-7 -7 -7 -6 -8 +0 +0 +0 +0 +0 +0 +0 +0 +0 -10 -8 -12 -8
-8
-
1.88E6.90E1.74E1.02E7.25E0.00E0.00E0.00E0.00E0.00E0.00E0.00E0.00E0.00E5.13E5.21E1.85E7.64E
AP [mol H+-Eq.] 5.67E
-2 -3 -2 -1 -3 +0 +0 +0 +0 +0 +0 +0 +0 +0 -5 -4 -7 -4
-4
-
9.14E7.41E4.61E2.76E3.89E0.00E0.00E0.00E0.00E0.00E0.00E0.00E0.00E0.00E9.39E1.00E9.24E5.30E
EP-freshwater [kg P-Eq.] 7.15E
-5 -6 -4 -5 -5 +0 +0 +0 +0 +0 +0 +0 +0 +0 -7 -6 -9 -6
-6
-
4.51E2.48E3.66E2.56E1.59E0.00E0.00E0.00E0.00E0.00E0.00E0.00E0.00E0.00E6.51E1.55E2.97E2.69E
EP-marine [kg N-Eq.] 1.21E
-3 -3 -3 -2 -3 +0 +0 +0 +0 +0 +0 +0 +0 +0 -6 -4 -8 -4
-4
-
5.18E2.74E4.03E2.85E1.78E0.00E0.00E0.00E0.00E0.00E0.00E0.00E0.00E0.00E8.02E1.71E4.59E3.03E
EP-terrestrial [mol N-Eq.] 1.37E
-2 -2 -2 -1 -2 +0 +0 +0 +0 +0 +0 +0 +0 +0 -5 -3 -7 -3
-3
-
1.34E7.37E1.12E7.50E5.12E0.00E0.00E0.00E0.00E0.00E0.00E0.00E0.00E0.00E2.04E5.23E9.13E8.44E
POCP [kg NMVOC-Eq.] 4.79E
-2 -3 -2 -2 -3 +0 +0 +0 +0 +0 +0 +0 +0 +0 -5 -4 -8 -4
-4
-
1.13E1.29E9.76E6.09E7.03E0.00E0.00E0.00E0.00E0.00E0.00E0.00E0.00E0.00E1.20E2.48E1.04E9.95E
ADPE [kg Sb-Eq.] 1.15E
-5 -6 -7 -6 -6 +0 +0 +0 +0 +0 +0 +0 +0 +0 -8 -7 -10 -8
-7
-
2.78E1.14E4.26E6.64E1.39E0.00E0.00E0.00E0.00E0.00E0.00E0.00E0.00E0.00E1.81E1.92E8.38E2.55E
ADPF [MJ] 2.29E
+1 +1 +1 +1 +1 +0 +0 +0 +0 +0 +0 +0 +0 +0 -1 +0 -4 +0
+0
-
[m³ world-Eq 1.40E3.85E8.39E1.38E3.73E0.00E0.00E0.00E0.00E0.00E0.00E0.00E0.00E0.00E2.03E5.35E3.28E8.00E
WDP 3.06E
deprived] +0 -2 -1 -1 -1 +0 +0 +0 +0 +0 +0 +0 +0 +0 -3 -3 -6 -3
-2
GWP = Global warming potential; ODP = Depletion potential of the stratospheric ozone layer; AP = Acidification potential of land and water; EP =
Caption Eutrophication potential; POCP = Formation potential of tropospheric ozone photochemical oxidants; ADPE = Abiotic depletion potential for non-
fossil resources; ADPF = Abiotic depletion potential for fossil resources; WDP = Water (user) deprivation potential
RESULTS OF THE LCA - INDICATORS TO DESCRIBE RESOURCE USE according to EN 15804+A2: 1 m2
Cementex / Cementex Extreme (10 mm)
Indicator Unit A1 A2 A3 A4 A5 B1/1 B1/2 B1/3 B2 B3 B4 B5 B6 B7 C1 C2 C3 C4 D
6.74E+1.39E-5.74E+6.47E-2.46E+0.00E+0.00E+0.00E+0.00E+0.00E+0.00E+0.00E+0.00E+0.00E+3.38E-2.66E-1.50E-1.09E-0.00E+
PERE [MJ]
0 1 0 1 0 0 0 0 0 0 0 0 0 0 2 2 4 1 0
-
1.57E+0.00E+4.38E+0.00E+ 0.00E+0.00E+0.00E+0.00E+0.00E+0.00E+0.00E+0.00E+0.00E+0.00E+0.00E+0.00E+0.00E+1.96E+
PERM [MJ] 2.70E+
1 0 0 0 0 0 0 0 0 0 0 0 0 0 0 0 0 0
0
-
2.24E+1.39E-1.01E+6.47E- 0.00E+0.00E+0.00E+0.00E+0.00E+0.00E+0.00E+0.00E+0.00E+3.38E-2.66E-1.50E-1.09E-1.96E+
PERT [MJ] 2.40E-
1 1 1 1 0 0 0 0 0 0 0 0 0 2 2 4 1 0
1
3.41E+1.17E+5.44E+6.65E+1.60E+0.00E+0.00E+0.00E+0.00E+0.00E+0.00E+0.00E+0.00E+0.00E+2.17E-1.93E+1.13E-2.68E+0.00E+
PENRE [MJ]
1 1 1 1 1 0 0 0 0 0 0 0 0 0 1 0 3 0 0
-
2.99E-0.00E+2.89E-0.00E+ 0.00E+0.00E+0.00E+0.00E+0.00E+0.00E+0.00E+0.00E+0.00E+0.00E+0.00E+0.00E+0.00E+3.65E-
PENRM [MJ] 2.87E-
1 0 1 0 0 0 0 0 0 0 0 0 0 0 0 0 0 2
1
3.44E+1.17E+5.47E+6.65E+1.57E+0.00E+0.00E+0.00E+0.00E+0.00E+0.00E+0.00E+0.00E+0.00E+2.17E-1.93E+1.13E-2.68E+3.65E-
PENRT [MJ]
1 1 1 1 1 0 0 0 0 0 0 0 0 0 1 0 3 0 2
5.40E-0.00E+0.00E+0.00E+0.00E+0.00E+0.00E+0.00E+0.00E+0.00E+0.00E+0.00E+0.00E+0.00E+0.00E+0.00E+0.00E+0.00E+1.37E+
SM [kg]
1 0 0 0 0 0 0 0 0 0 0 0 0 0 0 0 0 0 0
0.00E+0.00E+0.00E+0.00E+0.00E+0.00E+0.00E+0.00E+0.00E+0.00E+0.00E+0.00E+0.00E+0.00E+0.00E+0.00E+0.00E+0.00E+0.00E+
RSF [MJ]
0 0 0 0 0 0 0 0 0 0 0 0 0 0 0 0 0 0 0
0.00E+0.00E+0.00E+0.00E+0.00E+0.00E+0.00E+0.00E+0.00E+0.00E+0.00E+0.00E+0.00E+0.00E+0.00E+0.00E+0.00E+0.00E+0.00E+
NRSF [MJ]
0 0 0 0 0 0 0 0 0 0 0 0 0 0 0 0 0 0 0
-
3.15E-7.70E-1.50E-3.33E-9.27E-0.00E+0.00E+0.00E+0.00E+0.00E+0.00E+0.00E+0.00E+0.00E+1.33E-1.39E-2.48E-2.54E-
FW [m³] 9.89E-
2 4 2 3 3 0 0 0 0 0 0 0 0 0 4 4 7 3
4
PERE = Use of renewable primary energy excluding renewable primary energy resources used as raw materials; PERM = Use of
renewable primary energy resources used as raw materials; PERT = Total use of renewable primary energy resources; PENRE = Use of
non-renewable primary energy excluding non-renewable primary energy resources used as raw materials; PENRM = Use of non-
Caption
renewable primary energy resources used as raw materials; PENRT = Total use of non-renewable primary energy resources; SM = Use
of secondary material; RSF = Use of renewable secondary fuels; NRSF = Use of non-renewable secondary fuels; FW = Use of net fresh
water
RESULTS OF THE LCA – WASTE CATEGORIES AND OUTPUT FLOWS according to EN 15804+A2:
1 m2 Cementex / Cementex Extreme (10 mm)
Indicator Unit A1 A2 A3 A4 A5 B1/1 B1/2 B1/3 B2 B3 B4 B5 B6 B7 C1 C2 C3 C4 D
-
1.85E-2.91E-2.93E-1.11E-1.48E-0.00E+0.00E+0.00E+0.00E+0.00E+0.00E+0.00E+0.00E+0.00E+1.21E-5.04E-1.10E-3.03E-
HWD [kg] 5.46E-
5 5 5 4 5 0 0 0 0 0 0 0 0 0 7 6 9 6
6
-
3.92E-4.49E-4.56E-1.49E+8.87E-0.00E+0.00E+0.00E+0.00E+0.00E+0.00E+0.00E+0.00E+0.00E+6.39E-9.19E-3.74E-1.48E+
NHWD [kg] 1.43E-
1 1 1 0 1 0 0 0 0 0 0 0 0 0 4 2 6 1
2
-
9.30E-7.51E-5.20E-4.57E-4.79E-0.00E+0.00E+0.00E+0.00E+0.00E+0.00E+0.00E+0.00E+0.00E+1.28E-1.31E-3.38E-1.62E-
RWD [kg] 7.42E-
5 5 5 4 5 0 0 0 0 0 0 0 0 0 6 5 9 5
6
0.00E+0.00E+0.00E+0.00E+0.00E+0.00E+0.00E+0.00E+0.00E+0.00E+0.00E+0.00E+0.00E+0.00E+0.00E+0.00E+0.00E+0.00E+0.00E+
CRU [kg]
0 0 0 0 0 0 0 0 0 0 0 0 0 0 0 0 0 0 0
-
0.00E+0.00E+1.71E+0.00E+2.26E-0.00E+0.00E+0.00E+0.00E+0.00E+0.00E+0.00E+0.00E+0.00E+0.00E+0.00E+0.00E+0.00E+
MFR [kg] 1.94E+
0 0 0 0 1 0 0 0 0 0 0 0 0 0 0 0 0 0
0
0.00E+0.00E+0.00E+0.00E+0.00E+0.00E+0.00E+0.00E+0.00E+0.00E+0.00E+0.00E+0.00E+0.00E+0.00E+0.00E+0.00E+0.00E+0.00E+
MER [kg]
0 0 0 0 0 0 0 0 0 0 0 0 0 0 0 0 0 0 0
-
0.00E+0.00E+2.71E-0.00E+3.92E-0.00E+0.00E+0.00E+0.00E+0.00E+0.00E+0.00E+0.00E+0.00E+0.00E+0.00E+0.00E+0.00E+
EEE [MJ] 4.19E-
0 0 2 0 1 0 0 0 0 0 0 0 0 0 0 0 0 0
1
0.00E+0.00E+0.00E+0.00E+0.00E+0.00E+0.00E+0.00E+0.00E+0.00E+0.00E+0.00E+0.00E+0.00E+0.00E+0.00E+0.00E+0.00E+0.00E+
EET [MJ]
0 0 0 0 0 0 0 0 0 0 0 0 0 0 0 0 0 0 0
HWD = Hazardous waste disposed; NHWD = Non-hazardous waste disposed; RWD = Radioactive waste disposed; CRU = Components
Caption for re-use; MFR = Materials for recycling; MER = Materials for energy recovery; EEE = Exported electrical energy; EEE = Exported
thermal energy
RESULTS OF THE LCA – additional impact categories according to EN 15804+A2-optional:
1 m2 Cementex / Cementex Extreme (10 mm)
Indicator Unit A1 A2 A3 A4 A5 B1/1 B1/2 B1/3 B2 B3 B4 B5 B6 B7 C1 C2 C3 C4 D
-
[Disease 1.98E-6.71E-2.37E-2.30E-5.01E-0.00E 0.00E 0.00E 0.00E 0.00E 0.00E 0.00E 0.00E 0.00E1.34E-8.87E-8.48E-1.49E-
PM 6.10E-
Incidence] 7 8 7 7 8 +0 +0 +0 +0 +0 +0 +0 +0 +0 10 9 13 8
9
-
[kBq U235-8.03E-4.77E-3.68E-2.87E-4.03E-0.00E 0.00E 0.00E 0.00E 0.00E 0.00E 0.00E 0.00E 0.00E1.56E-8.40E-2.64E-1.05E-
IRP 7.80E-
Eq.] 2 2 2 1 2 +0 +0 +0 +0 +0 +0 +0 +0 +0 3 3 6 2
3
-
8.55E 9.96E 2.01E 4.76E 1.73E 0.00E 0.00E 0.00E 0.00E 0.00E 0.00E 0.00E 0.00E 0.00E1.24E-1.54E7.23E-1.54E
ETP-fw [CTUe] 1.90E
+1 +0 +1 +1 +1 +0 +0 +0 +0 +0 +0 +0 +0 +0 1 +0 4 +0
+0
-
2.68E-4.40E-1.02E-2.34E-3.21E-0.00E 0.00E 0.00E 0.00E 0.00E 0.00E 0.00E 0.00E 0.00E3.20E-4.32E-2.25E-3.69E-
HTP-c [CTUh] 1.79E-
9 10 9 9 9 +0 +0 +0 +0 +0 +0 +0 +0 +0 12 11 14 11
10
-
6.62E-1.12E-2.85E-4.53E-1.89E-0.00E 0.00E 0.00E 0.00E 0.00E 0.00E 0.00E 0.00E 0.00E1.09E-1.68E-6.65E-9.96E-
HTP-nc [CTUh] 1.83E-
8 8 8 8 8 +0 +0 +0 +0 +0 +0 +0 +0 +0 10 9 13 10
9
-
1.00E 7.49E 7.80E 2.52E 9.15E 0.00E 0.00E 0.00E 0.00E 0.00E 0.00E 0.00E 0.00E 0.00E4.42E-1.33E6.26E-4.85E
SQP [-] 3.34E
+2 +0 +1 +1 +0 +0 +0 +0 +0 +0 +0 +0 +0 +0 2 +0 4 +0
+1
PM = Potential incidence of disease due to PM emissions; IR = Potential Human exposure efficiency relative to U235; ETP-fw = Potential
Caption comparative Toxic Unit for ecosystems; HTP-c = Potential comparative Toxic Unit for humans (cancerogenic); HTP-nc = Potential
comparative Toxic Unit for humans (not cancerogenic); SQP = Potential soil quality index
7 Environmental Product Declaration Etex – Cementex/Cementex Extreme
Disclaimer 1 – for the indicator “Potential Human exposure efficiency relative to U235”. This impact category
deals mainly with the eventual impact of low-dose ionizing radiation on human health of the nuclear fuel cycle. It
does not consider effects due to possible nuclear accidents, occupational exposure or radioactive waste disposal
in underground facilities. Potential ionizing radiation from the soil, radon and from some construction materials is
also not measured by this indicator.
Disclaimer 2 – for the indicators “abiotic depletion potential for non-fossil resources”, “abiotic depletion potential
for fossil resources”, “water (user) deprivation potential, deprivation-weighted water consumption”, “potential
comparative toxic unit for ecosystems”, “potential comparative toxic unit for humans – cancerogenic”, “Potential
comparative toxic unit for humans - not cancerogenic”, “potential soil quality index”. The results of this
environmental impact indicator shall be used with care as the uncertainties on these results are high as there is
limited experience with the indicator.
References
Standards: Candidate List of substances of very high concern for
Authorisation. Available at:
CEN/TR 16970:2016 <https://echa.europa.eu/candidate-list-table>.
CEN/TR 16970:2016 Sustainability of construction
works - Guidance for the implementation of EN 15804 CPR
European Regulation N° 305/2011 (CPR)
EN 12467:2013+A2:2018
EN 12467:2013...Fibre-cement flat sheets - Product Enperas project report of Etex: Life cycle assessment
specification and test methods of Cementex / Cementex Extreme; October 2022,
author(s): Varun Gowda Palahalli Ramesh.
EN 15804:2012+A2:2019+AC:2021.
EN 15804:2012…Sustainability of construction works – IBU 2021
Environmental product declarations – Core rules for Institut Bauen und Umwelt e.V.: General Instructions
the product category of construction products. for the EPD programme of Institut Bauen und Umwelt
European standard. e.V., Version 2.0, Berlin: Institut Bauen und Umwelt
e.V., 2021. www.ibu-epd.com
EN 13501-1
EN 13501-1 Fire classification of construction products JRC. 2018. https://eplca.jrc.ec.europa.eu/ELCD3/
and building elements - Part 1: Classification using
data from reaction to fire tests NBN/DTD B 08-001:2017. Delem L., Wastiels L. 2016.
B-PCR. Sustainability of construction works –
ISO 9000 Environmental product declarations – Core rules for
ISO 9000 family of Quality management systems the product category of construction products –
National annex to NBN EN 15804+A1.
ISO 13787:2003
ISO 13787:2003 Thermal insulation products for PCR Part A, Calculation Rules for the Life Cycle
building equipment and industrial installations — Assessment and Requirements on the Project Report
Determination of declared thermal conductivity according to EN 15804+A2:2019, Version 1.2, Institut
Bauen und Umwelt e.V., www.ibu-epd.com, 2021
ISO 14001:2015
ISO 14001:2015 Environmental management systems PCR Part B, Requirements on the EPD for Fibre
— Requirements with guidance for use cement / Fibre concrete, Version 1.7, Institut Bauen
und Umwelt e.V., www.bau-umwelt.com, 2019
ISO 14025:2011
Environmental labels and declarations - Type III Pré Consultants (2021). SimaPro 9.2.0.1 [Computer
environmental declarations - Principles and procedures Software]. Amersfoort, The Netherlands in combination
with a specific LCA software for ETEX. Database used
ISO 14040:2006 was Ecoinvent 3.6
ISO 14040:2006 Environmental management – Life
cycle assessment – Principles and framework. Servaes, R., Allacker, K., Debacker, W., Delem L., De
Nocker, L., De Troyer, F. Janssen, A., Peeters, K.,
ISO 14044:2006 Spirinckx, C., Van Dessel, J. (2013). Milieuprofiel van
ISO 14044:2006Environmental management – Life gebouwelementen. Te raadplegen via:
cycle assessment – Requirements and guidelines. www.ovam.be/materiaalprestatie-gebouwen.
ISO 45001 Technical Data Sheet of Cementex and Cementex
ISO 45001 Occupational Health and Safety Extreme (https://www.siniat.si/-/dam/cementex-tehnini-
Management Systems list-siniat/pi52988/original/cementex-siniat-tehnicni-list-
siniat.pdf?v=19900
Further References:
Wernet, G., Bauer, C., Steubing, B., Reinhard, J.,
Moreno-Ruiz, E., and Weidema, B., 2016. The
ecoinvent database version 3 (part I): overview and
8 Environmental Product Declaration Etex – Cementex/Cementex Extreme
methodology. The International Journal of Life Cycle
Assessment, [online] 21(9), pp.1218–1230. Available
at: <http://link.springer.com/10.1007/s11367-016-1087-
8>.
9 Environmental Product Declaration Etex – Cementex/Cementex Extreme
Publisher
Institut Bauen und Umwelt e.V. Tel +49 (0)30 3087748- 0
Hegelplatz 1 Fax +49 (0)30 3087748- 29
10117 Berlin Mail info@ibu-epd.com
Germany Web www.ibu-epd.com
Programme holder
Institut Bauen und Umwelt e.V. Tel +49 (0)30 - 3087748- 0
Hegelplatz 1 Fax +49 (0)30 – 3087748 - 29
10117 Berlin Mail info@ibu-epd.com
Germany Web www.ibu-epd.com
Author of the Life Cycle
Assessment Tel +32 3 376 00 19
Enperas Fax -
Thorpark 8300 Mail info@enperas.com
3600 Genk Web https://www.enperas.com/en/
Belgium
Owner of the Declaration
Etex Building Performance Tel +32 2 778 12 11
International Fax +32 2 778 12 12
Rue Marcel Demonque 500 Mail info@etexgroup.com
84915 Avignon Cedex 9 Web http://www.etexgroup.com
France
