ENVIRONMENTAL PRODUCT DECLARATION
as per ISO 14025 and EN 15804+A2
Owner of the Declaration dormakaba International Holding GmbH
Publisher Institut Bauen und Umwelt e.V. (IBU)
Programme holder Institut Bauen und Umwelt e.V. (IBU)
Declaration number EPD-DOR-20220205-CBA5-EN
Issue date 18.10.2022
Valid to 17.10.2027
Charon 20 - Half Height Swing Doors
dormakaba
www.ibu-epd.com | https://epd-online.com
General Information
dormakaba Charon 20 - Half Height Swing Doors
Programme holder Owner of the declaration
IBU – Institut Bauen und Umwelt e.V. dormakaba International Holding GmbH
Hegelplatz 1 DORMA Platz 1
10117 Berlin 58256 Ennepetal
Germany Germany
Declaration number Declared product / declared unit
EPD­DOR­20220205­CBA5­EN 1 dormakaba Charon 20 ­ Half Height Swing Door, consisting of the
following items:­ control system Charon 20
­ power supply unit
­ power supply accessories
­ profile
­ profile covers
­ engine
­ door leaf ESG
­ product packaging
This declaration is based on the product category rules: Scope:
Electronic and physical Access Control Systems, 01.08.2021 This EPD is a specific product decalaration for the Charon 20 ­ Half Height
(PCR checked and approved by the SVR) Swing Door.
The underlying life cycle assessment is based on the entire life cycle of
this specific Charon 20 swing door.
Issue date The products are manufactured at the dormakaba production facility in
Bühl (Germany).
18.10.2022
Green electricity is being used at this production site.
Data represents the year 2022.
Valid to
The owner of the declaration shall be liable for the underlying information
17.10.2027 and evidence; the IBU shall not be liable with respect to manufacturer
information, life cycle assessment data and evidences.
The EPD was created according to the specifications of EN 15804+A2. In
the following, the standard will be simplified as EN 15804.
Verification
The standard EN 15804 serves as the core PCR
Independent verification of the declaration and data according to ISO
14025:2011
internally X externally
Dipl.­Ing. Hans Peters
(Chairman of Institut Bauen und Umwelt e.V.)
Florian Pronold Dr.­Ing. Wolfram Trinius,
(Managing Director Institut Bauen und Umwelt e.V.) (Independent verifier)
1 Environmental Product Declaration ­ dormakaba ­ Charon 20 ­ Half Height Swing Doors
Product
Please provide a general indication of the area of use of the
Product description/Product definition device (indoor or outdoor).
Charon 20 - Half Height Swing Doors
Dimensions of Charon 20 - Half Height Swing Doors
Opening on demand with the Charon 20 swing door.
The Charon swing door can be installed directly on the housing Name Value Unit
of the Argus sensor barrier. It provides extended passage width Power supply max. 240 V
with a clear opening of up to 900 mm to accommodate Drive unit Diameter 75 mm
wheelchairs or material trolleys.
Upper edge of the drive unit Dimension 850 mm
Door leaf radius Dimension 900 mm
The shape, surface and colour of the Charon 20 swing door
precisely matches that of the sensor barrier to which it is bolted. Upper edge of the door leaf Dimension 990 mm
The Charon 20 - Half Height Swing Door includes the
This solution enables a visually appealing and easy­to­ following components:
implement opening, as electrical components are integrated ­ control unit
into the housing of the Argus sensor barrier and the cables are ­ power back
routed through it. No additional cable bores and cable routing ­ cover profile
are therefore required in the installation area. For the placing ­ glass door leaves ESG
on the market in the European Union/European Free Trade ­ drive unit
Associaton (EU/EFTA) (with the exception of Switzerland) the
following legal provisions apply: The total weight of all components is 26,10 kg including
• Machinery Directive 2006/42/EC packaging 32,31 kg.
• 2014/30/EU Electromagnetic Compatibility Directive
• 2011/65/EU RoHS3 Directive Product not harmonised in accordance with the
• DIN EN ISO 12100:2011-03 Safety of machinery CPR but in accordance with other provisions for harmonisation
• DIN EN 16005: 2013-01 and Amendment 2015-10 of the EU:
Power operated pedestrian doorsets
• DIN EN ISO 13849- 1:2016-06 Safety of machinery
• DIN EN ISO 13849- 2:2013-02 Safety of machinery • Machinery Directive 2006/42/EC
• DIN EN 60335-2-103: 2016-05 Household and similar • 2014/30/EU Electromagnetic Compatibility Directive
electrical appliances • 2011/65/EU ROHS2 Directive
• DIN EN 61000-3-2:2015-03 Electromagnetic • DIN EN ISO 12100:2011-03 Safety of machinery
compatibility (EMC) • DIN EN 16005: 2013-01 and Amendment 2015-10
• DIN EN 61000-6-2: 2005 and Amendment:2011 Power operated pedestrian doorsets
Electromagnetic Compatibility (EMC) • DIN EN ISO 13849- 1:2016-06 Safety of machinery
• DIN EN 61000-6-3:2007 and A1:2011 Electromagnetic • DIN EN ISO 13849- 2:2013-02 Safety of machinery
Compatibility (EMC) • DIN EN 60335-2-103: 2016-05 Household and similar
The CE­marking takes into account the proof of conformity with electrical appliances
the respective harmonized standards based on the legal • DIN EN 61000-3-2:2015-03 Electromagnetic
provisions above. compatibility (EMC)
• DIN EN 61000-6-2: 2005 and Amendment:2011
For the application and use the respective national provisions Electromagnetic Compatibility (EMC)
apply. • DIN EN 61000-6-3:2007 and A1:2011 Electromagnetic
Compatibility (EMC)
Application
Charon 20 ­ Half Height Swing Doors can be used for Base materials/Ancillary materials
convenient entry into: For the main Charon 20 swing door product components the
• Office and administrative buildings composition is the following.
• Ministries and government buildings
• Banks and financial institutions
• Industrial buildings The composition is listed in the following table:
• Schools and universities
Technical Data
The technical specifications of the products within the scope of
the EPD shall be listed, including the reference to the test
methods/test standards for each specification.
For products with CE marking, the technical specifications must
be specified in accordance with information in the declaration of
performance. The properties relevant to the product should be
specified in the table below. If no information is given for
properties, an explanation must be given in the background
report to the EPD as to why the property is not relevant to the The product contains partial articles which contain substances
product. listed in the Candidate List of REACH Regulation
1907/2006/EC (date: 10.06.2022) exceeding 0.1 percentage by
2 Environmental Product Declaration ­ dormakaba ­ Charon 20 ­ Half Height Swing Doors
mass: yes
Reference service life
The life cycle of an Charon 20 ­ Half Height Swing Door is
• Lead (Pb): 7439­92­1 (CAS­No.) is included in some of
about 15 years, depending on the application and frequency of
the alloys used. The concentration of lead in each
use. The Charon 20 swing door is tested according to EN
individual alloy does not exceed 0,35 %(by mass).
16005.
The Candidate List can be found on the /ECHA/ website
address: https://echa.europa.eu/de/home.
LCA: Calculation rules
Declared Unit Use stage - Module B6
The declared unit is 1 piece of product: 26.10 kg The use stage related to the operation of the building includes:
Name Value Unit — B6, operational energy use
Declared unit 1 pce.
End-of-life stage– Modules C1-C4 and D
Mass (total system excluding packaging) 26.1 kg
The end­of­life stage includes:
— C1, de­construction, demolition;
System boundary
— C2, transport to waste processing;
Type of EPD:
— C3, waste processing for reuse, recovery and/or recycling;
cradle to gate with options, modules C1–C4, and module D
— C4, disposal; including provision and all transport, provision
(A1–A3 + C + D and additional modules: A4 + A5 + B6)
of all materials, products and related energy and water use.
— D, (Benefits and loads beyond the system boundary)
Production - Module A1-A3
includes: recycling potentials, expressed as net impacts and
The product stage includes:
benefits.
— A1, raw material extraction, processing and mechanical
treatments, processing of secondary material input (e.g. Geographic Representativeness
recycling processes), Land or region, in which the declared product system is
— A2, transport to the manufacturer, manufactured, used or handled at the end of the product´s
— A3, manufacturing and assembly including provision of all lifespan: Germany
materials, products and energy, as well as waste processing up
to the end­of waste state.
Comparability
Construction stage - Modules A4-A5 Basically, a comparison or an evaluation of EPD data is only
The construction process stage includes: possible if all the data sets to be compared were created
— A4, transport to the building site; according to EN 15804 and the building context, respectively
— A5, installation into the building; including provision of all the product­specific characteristics of performance, are taken
materials, products and energy, as well as waste processing up into account.
to the end of waste state or disposal of final residues during the
construction process stage.
LCA: Scenarios and additional technical information
Name Value Unit
Characteristic product properties of biogenic carbon
Days per year in use 365 days
Information on describing the biogenic Carbon Content at On mode per day 1 hours
factory gate
Idle mode per day 23 hours
Name ValueUnit
On mode power 20 W
Biogenic carbon content in accompanying kg
2.29 Idle mode power 3 W
packaging C
Electricity consumption (per 1 year) 32,485 kWh
The following technical scenario information is required for the End of life (C1-C4)
declared modules Name Value Unit
Transport to the building site (A4) Collected separately waste type 29.1 kg
Name Value Unit Recycling 4.8 kg
Litres of fuel (per 1 kg) 0.00276 l/100km Energy recovery 0.838 kg
Capacity utilisation (including empty runs) 55 % Landfilling 23.5 kg
Transport distance via medium truck 100 km Transport to waste management 50 km
The product is disassembled in a recycling process. Material
Reference service life
recycling is then assumed for the metals and electronics. The
Name Value Unit
plastic components are assumed to be incinerated with energy
Life Span according to the manufacturer 15 a recovery. Glass and electro mechanics (e.g. cable, connector)
are landfilled.
Operational energy use (B6)
Region for the End of Life is: Global.
The use stage is declared for 15 years
Reuse, recovery and/or recycling potentials (D), relevant
scenario information
3 Environmental Product Declaration ­ dormakaba ­ Charon 20 ­ Half Height Swing Doors
Collection rate is 100%.
4 Environmental Product Declaration ­ dormakaba ­ Charon 20 ­ Half Height Swing Doors
LCA: Results
DESCRIPTION OF THE SYSTEM BOUNDARY (X = INCLUDED IN LCA; MND = MODULE OR INDICATOR NOT DECLARED; MNR
= MODULE NOT RELEVANT)
Benefits and
Construction loads beyond
Product stage Use stage End of life stage
process stage the system
boundaries
la ire ta m w a Ry lp p u s tro p s n a rT g n iru tc a fu n a M e h t m o rf tro p s n a rTe tis e h t o t e ta g y lb m e s s A e s U e c n a n e tn ia M ria p e R tn e m e c a lp e R tn e m h s ib ru fe R y g re n e la n o ita re p Oe s u re ta w la n o ita re p Oe s u n o itc u rts n o c ­e Dn o itilo m e d tro p s n a rT g n is s e c o rp e ts a W la s o p s iD ­e s u e R­y re v o c e R­g n ilc y c e Rla itn e to p
A1 A2 A3 A4 A5 B1 B2 B3 B4 B5 B6 B7 C1 C2 C3 C4 D
X X X X X MND X MNR MNR MNR X MND X X X X X
RESULTS OF THE LCA - ENVIRONMENTAL IMPACT according to EN 15804+A2: 1 piece Charon 20 Half-Height Swing Door
Parameter Unit A1-A3 A4 A5 B2 B6 C1 C2 C3 C4 D
GWP­total kg CO 2 eq 8.8E+01 2.83E­01 8.81E+00 0 1.97E+02 0 1.28E­01 2.13E+00 4.84E­09 ­3.09E+01
GWP­fossil kg CO 2 eq 9.76E+01 2.7E­01 2.21E­01 0 1.96E+02 0 1.23E­01 2.13E+00 3E­03 ­3.08E+01
GWP­
biogenic kg CO 2 eq ­9.63E+00 1.2E­02 8.58E+00 0 6.54E­01 0 6E­03 4.96E­05 3.71E­01 ­6.2E­02
GWP­luluc kg CO 2 eq 8.41E­02 6.43E­06 1.45E­04 0 2.84E­01 0 2.92E­06 1.2E­04 3.21E­11 ­1.4E­02
ODP kg CFC11 eq 1.78E­09 2.85E­17 1.59E­15 0 4.32E­12 0 1.29E­17 1.07E­15 3.25E­09 ­1.81E­10
AP mol H+ eq 6.11E­01 2.7E­04 2E­03 0 4.33E­01 0 1.23E­04 3.79E­04 2.96E­01 ­1.33E­01
EP­
kg P eq 3.27E­04 5.78E­08 3.1E­07 0 5.24E­04 0 2.62E­08 1.71E­07 6.11E­07 ­1.94E­05
freshwater
EP­marine kg N eq 1.01E­01 8.6E­05 8.9E­04 0 9.6E­02 0 3.9E­05 8.55E­05 6.57E­04 ­1.7E­02
EP­terrestrial mol N eq 1.11E+00 9.56E­04 1.1E­02 0 1.01E+00 0 4.34E­04 2E­03 7E­03 ­1.82E­01
kg NMVOC
POCP 2.67E­01 2.43E­04 2E­03 0 2.64E­01 0 1.1E­04 2.37E­04 2E­03 ­5.2E­02
eq
ADPE kg Sb eq 5.01E­03 8.1E­09 2.51E­08 0 5.68E­05 0 3.67E­09 1.47E­08 3.2E­08 ­7.41E­04
ADPF MJ 1.25E+03 3.83E+00 2.78E+00 0 3.45E+03 0 1.74E+00 9.87E­01 4.67E+00 ­4.44E+02
m3 world eq
WDP 1.8E+01 5.29E­04 1.09E+00 0 4.28E+01 0 2.4E­04 2.18E­01 3.7E­02 ­3.11E+00
deprived
GWP = Global warming potential; ODP = Depletion potential of the stratospheric ozone layer; AP = Acidification potential of land and water; EP =
Eutrophication potential; POCP = Formation potential of tropospheric ozone photochemical oxidants; ADPE = Abiotic depletion potential for non­fossil
resources; ADPF = Abiotic depletion potential for fossil resources; WDP = Water (user) deprivation potential)
RESULTS OF THE LCA - INDICATORS TO DESCRIBE RESOURCE USE according to EN 15804+A2: 1 piece Charon 20 Half-
Height Swing Door
Parameter Unit A1-A3 A4 A5 B2 B6 C1 C2 C3 C4 D
PERE MJ 6.39E+02 1.2E­02 7.5E+01 0 1.53E+03 0 5E­03 2.57E­01 6.12E­01 ­1.8E+02
PERM MJ 7.45E+01 0 ­7.45E+01 0 0 0 0 0 0 0
PERT MJ 7.14E+02 1.2E­02 5.05E­01 0 1.53E+03 0 5E­03 2.57E­01 6.12E­01 ­1.8E+02
PENRE MJ 1.22E+03 3.83E+00 2.78E+00 0 3.45E+03 0 1.74E+00 3.06E+01 4.67E+00 ­4.44E+02
PENRM MJ 2.96E+01 0 0 0 0 0 0 ­2.96E+01 0 0
PENRT MJ 1.25E+03 3.83E+00 2.78E+00 0 3.45E+03 0 1.74E+00 9.88E­01 4.67E+00 ­4.44E+02
SM kg 4.52E+00 0 0 0 0 0 0 0 0 0
RSF MJ 0 0 0 0 0 0 0 0 0 0
NRSF MJ 0 0 0 0 0 0 0 0 0 0
FW m3 8.65E­01 2.17E­05 2.6E­02 0 1.77E+00 0 9.83E­06 5E­03 1E­03 ­3.51E­01
PERE = Use of renewable primary energy excluding renewable primary energy resources used as raw materials; PERM = Use of renewable primary
energy resources used as raw materials; PERT = Total use of renewable primary energy resources; PENRE = Use of non­renewable primary energy
excluding non­renewable primary energy resources used as raw materials; PENRM = Use of non­renewable primary energy resources used as raw
materials; PENRT = Total use of non­renewable primary energy resources; SM = Use of secondary material; RSF = Use of renewable secondary fuels;
NRSF = Use of non­renewable secondary fuels; FW = Use of net fresh water
RESULTS OF THE LCA – WASTE CATEGORIES AND OUTPUT FLOWS according to EN 15804+A2:
1 piece Charon 20 Half-Height Swing Door
Parameter Unit A1-A3 A4 A5 B2 B6 C1 C2 C3 C4 D
HWD kg 1.76E­05 3.72E­10 4.1E­09 0 1.43E­06 0 1.69E­10 3.76E­09 7.12E­08 ­1.83E­07
NHWD kg 1.5E+01 3.92E­04 2.76E­01 0 2.45E+00 0 1.78E­04 2.21E­01 2.35E+01 ­6.64E+00
RWD kg 5.2E­02 4.12E­06 1.46E­04 0 5.23E­01 0 1.87E­06 3.66E­05 5.32E­05 ­4.2E­02
CRU kg 0 0 0 0 0 0 0 0 0 0
MFR kg 0 0 0 0 0 0 0 5.01E+00 0 0
MER kg 0 0 0 0 0 0 0 0 0 0
EEE MJ 0 0 1.33E+01 0 0 0 0 0 0 0
5 Environmental Product Declaration ­ dormakaba ­ Charon 20 ­ Half Height Swing Doors
EET MJ 0 0 2.42E+01 0 0 0 0 0 0 0
HWD = Hazardous waste disposed; NHWD = Non­hazardous waste disposed; RWD = Radioactive waste disposed; CRU = Components for re­use;
MFR = Materials for recycling; MER = Materials for energy recovery; EEE = Exported electrical energy; EET = Exported thermal energy
RESULTS OF THE LCA – additional impact categories according to EN 15804+A2-optional:
1 piece Charon 20 Half-Height Swing Door
Parameter Unit A1-A3 A4 A5 B2 B6 C1 C2 C3 C4 D
Disease
PM 5.48E­06 1.42E­09 1.37E­08 0 3.63E­06 0 6.45E­10 4.84E­09 3.16E­08 ­1.97E­06
incidence
IR kBq U235 eq 8.76E+00 5.88E­04 2.3E­02 0 8.59E+01 0 2.67E­04 3E­03 5E­03 ­8.31E+00
ETP­fw CTUe 9.52E+02 2.72E+00 1.32E+00 0 1.48E+03 0 1.23E+00 3.71E­01 2.67E+00 ­1.65E+02
HTP­c CTUh 1.28E­06 5.11E­11 6.98E­11 0 4.08E­08 0 2.32E­11 3.21E­11 3.95E­10 ­1.48E­08
HTP­nc CTUh 3.72E­06 2.18E­09 3.02E­09 0 1.5E­06 0 9.91E­10 3.25E­09 4.36E­08 ­2.26E­07
SQP SQP 1.46E+03 1E­02 7.37E­01 0 1.1E+03 0 4E­03 2.96E­01 9.73E­01 ­2.86E+01
PM = Potential incidence of disease due to PM emissions; IR = Potential Human exposure efficiency relative to U235; ETP­fw = Potential comparative
Toxic Unit for ecosystems; HTP­c = Potential comparative Toxic Unit for humans (cancerogenic); HTP­nc = Potential comparative Toxic Unit for humans
(not cancerogenic); SQP = Potential soil quality index
Disclaimer 1 – for the indicator 'Potential Human exposure efficiency relative to U235'. This impact category deals mainly with the
eventual impact of low­dose ionizing radiation on human health of the nuclear fuel cycle. It does not consider effects due to possible
nuclear accidents, occupational exposure or radioactive waste disposal in underground facilities. Potential ionizing radiation from the
soil, radon and from some construction materials is also not measured by this indicator.
Disclaimer 2 – for the indicators 'abiotic depletion potential for non­fossil resources', 'abiotic depletion potential for fossil resources',
'water (user) deprivation potential, deprivation­weighted water consumption', 'potential comparative toxic unit for ecosystems', 'potential
comparative toxic unit for humans – cancerogenic', 'Potential comparative toxic unit for humans ­ not cancerogenic', 'potential soil
quality index'.
The results of this environmental impact indicator shall be used with care as the uncertainties on these results are high as there is
limited experience with the indicator.
References
Standards DIN EN ISO 13849- 1
DIN EN ISO 13849­ 1:2016­06 Safety of machinery
EN 15804
EN 15804:2012+A1 2013, Sustainability of construction works DIN EN ISO 13849- 2
— Environmental Product Declarations — Core rules for the DIN EN ISO 13849­ 2:2013­02 Safety of machinery
product category of construction products.
ISO 14025
EN 15804 DIN EN ISO 14025:2011­10, Environmental labels and
EN 15804:2012+A2:2019+AC:2021, Sustainability of declarations — Type III environmental declarations —
construction works — Environmental Product Declarations — Principles and procedures.
Core rules for the product category of construction products.
EN 15804
ISO 14025 EN 15804+A2: 2019+AC:2021, Sustainability of construction
EN ISO 14025:2011, Environmental labels and declarations — works — Environmental Product Declarations — Core rules for
Type III environmental declarations — Principles and the product category of construction products.
procedures.
Further References DIN EN 16005
DIN EN 16005:
IBU 2021 2013­01 and Amendment 2015­10 Power operated pedestrian
Institut Bauen und Umwelt e.V.: General Instructions for the doorsets
EPD programme of Institut Bauen und Umwelt e.V., Version
2.0, Berlin: Institut Bauen und Umwelt e.V., 2021 DIN EN 60335-2
www.ibu­epd.com DIN EN 60335­2­103: 2016­05 Household and similar electrical
appliances
Machinery Directive 2006/42/EC DIN EN 61000-3-2
DIRECTIVE 2006/42/EC OF THE EUROPEAN PARLIAMENT DIN EN 61000­3­2:2015­03 Electromagnetic compatibility
AND OF THE COUNCILof 17 May 2006on machinery, and (EMC)
amending Directive 95/16/EC
DIN EN 61000-6-2
Electromagnetic Compatibility Directive 2014/30/EU DIN EN 61000­6­2: 2005 and Amendment:2011
DIRECTIVE 2014/30/EU OF THE EUROPEAN PARLIAMENT Electromagnetic Compatibility (EMC)
AND OF THE COUNCILof 26 February 2014on the
harmonisation of the laws of the Member States relating to DIN EN 61000-6-3
electromagnetic compatibility DIN EN 61000­6­3:2007 and A1:2011 Electromagnetic
Compatibility (EMC)
DIN EN ISO 12100
DIN EN ISO 12100:2011­03 Safety of machinery REACH
Regulation (EC) No 1907/2006 of the European Parliament and
6 Environmental Product Declaration ­ dormakaba ­ Charon 20 ­ Half Height Swing Doors
of the Council on the Registration, Evaluation, Authorisation GaBi life cycle inventory data documentation
and Restriction of Chemicals (REACH) (https://www.gabisoftware.
com/support/gabi/gabidatabase[1]2020­lci­documentation/).
ISO 9001
ISO 9001:2015­09 Quality management systems ­ LCA-tool dormakaba
Requirements LCA tool, ESC (Entrance System Control)
Tool No.: IBU­DOR­202109­LT1­EN Developed by Sphera
European Waste Catalogue (EWC) Solutions GmbH
COMMISSION DECISION of 18 December 2014 amending
Decision 2000/532/EC on the list of waste pursuant to Directive PCR Part A
2008/98/EC of the European Parliament and of the Council PCR – Part A: Calculation Rules for the Life Cycle Assessment
and Requirements on the Project Re­port according to EN
Further References 15804+A2:2019, Version 1.0, Institut Bauen und Umwelt e.V.,
www.ibu­epd.com, 2020.
GaBi ts software
Sphera Solutions GmbH Gabi Software System and Database PCR Part B
for Life Cycle Engineering 1992­2020 Version 10.0.0.71 PCR – Part B:
University of Stuttgart Leinfelden­Echterdingen Requirements on the EPD for electronic and physical Access
Control Systems, version 1.2, Institut Bauen und Umwelt e.V.,
GaBi ts documentation www.ibu­epd.com, 2019.
7 Environmental Product Declaration ­ dormakaba ­ Charon 20 ­ Half Height Swing Doors
Publisher
Institut Bauen und Umwelt e.V. +49 (0)30 3087748­ 0
Hegelplatz 1 info@ibu­epd.com
10117 Berlin www.ibu­epd.com
Germany
Programme holder
Institut Bauen und Umwelt e.V. +49 (0)30 3087748­ 0
Hegelplatz 1 info@ibu­epd.com
10117 Berlin www.ibu­epd.com
Germany
Author of the Life Cycle Assessment
Sphera Solutions GmbH +49 711 341817­0
Hauptstraße 111­ 113 info@sphera.com
70771 Leinfelden­Echterdingen www.sphera.com
Germany
Owner of the Declaration
dormakaba International Holding GmbH +49 2333 793­0
DORMA Platz 1 info.de@dormakaba.com
58256 Ennepetal www.dormakaba.com
Germany
8 Environmental Product Declaration ­ dormakaba ­ Charon 20 ­ Half Height Swing Doors
