ENVIRONMENTAL PRODUCT DECLARATION
as per ISO 14025 and EN 15804+A1
Owner of the Declaration NMC S.A.
Programme holder Institut Bauen und Umwelt e.V. (IBU)
Publisher Institut Bauen und Umwelt e.V. (IBU)
Declaration number EPD-NMC-20210315-IBD1-EN
Issue date 05.01.2022
Valid to 04.01.2027
CLIMAFLEX® SPIRAL
NMC S.A.
www.ibu-epd.com | https://epd-online.com
Umwelt Produktdeklaration Name des Herstellers – Name des Produkts
1. General Information
NMC S.A. CLIMAFLEX® SPIRAL
Programme holder Owner of the declaration
IBU – Institut Bauen und Umwelt e.V. NMC S.A.
Panoramastr. 1 Gert-Noel Strasse
10178 Berlin BE-4731 Eynatten
Germany
Declaration number Declared product / declared unit
EPD-NMC-20210315-IBD1-EN 1 m³ insulation material CLIMAFLEX® SPIRAL
This declaration is based on the product Scope:
category rules: Product line CLIMAFLEX® SPIRAL
Insulating materials made of foam plastics, 01.2019 Self supporting ventilation pipe made of polyethene
(PCR checked and approved by the SVR) foam (PEF). This declaration is an Environmental
Product Declaration according to /ISO14025/
describing the specific environmental performance of
Issue date
the product produced in Belgium at the site of
05.01.2022
Eynatten.
Valid to
The owner of the declaration shall be liable for the
04.01.2027
underlying information and evidence; the IBU shall not
be liable with respect to manufacturer information, life
cycle assessment data and evidences.
The EPD was created according to the specifications
of EN 15804+A1. In the following, the standard will be
simplified as EN 15804.
Verification
The standard EN 15804 serves as the core PCR
Independent verification of the declaration and data
according to ISO 14025:2010
Dipl. Ing. Hans Peters internally x externally
(chairman of Institut Bauen und Umwelt e.V.)
Dr. Alexander Röder Vito D'Incognito
(Managing Director Institut Bauen und Umwelt e.V.)) (Independent verifier)
2. Product
2.1 Product description/Product definition  Products made of PE foam yield a good
CLIMAFLEX® SPIRAL is a professional bio- cost/performance ratio.
polyethylene-based closed-cell foam for self-
 Polyethylene Foam is corrosion resistant and
supporting ventilation pipes for interior use. Its low
its good thermal and acoustic insulation
weight, its corrosion resistance and its good thermal
and acoustic insulation, coupled with the fact that it is allows having a good alternative to
simple and quick to fit, make CLIMAFLEX® SPIRAL a conventional ventilation pipes.
worthwhile alternative to conventional ventilation
pipes. CLIMAFLEX® SPIRAL provides solutions that
follow all necessary guidelines and standards for any
2.3 Technical Data
type of installation. For the placing on the market of the
product in the European Union/European Free Trade
Association (EU/EFTA) (with the exception of
Performance data of the product in accordance with
Switzerland) - Thermal Insulation products for building
the Declaration of Performance with respect to its
equipment and industrial installations. Factory made
Essential Characteristics according to /EN 14313/
polyethylene foam (PEF) and the CE-marking. For the
apply. Further data:
application and use, the respective national provisions
Name Value Unit
apply.
Gross density 30 kg/m3
Thermal conductivity at 40 °C 0.048 W/(mK)
2.2 Application
Max Service Temperature Acc. to
CLIMAFLEX® SPIRAL are used as self-supporting 100 °C
/EN 14707
ventilation pipes for interior use in industrial
Min Service Temperature 0 °C
installations and building equipment
Water absorption Acc. to EN
 Polyethylene foam is a cost-efficient material WS005
13472
with good insulating properties.
2 Environmental Product Declaration NMC sa – CLIMAFLEX® SPIRAL
Traces quantities of water soluble form a flowable thermoplastic mass. The thermoplastic
Cl15 - F10
ions and pH-value Acc. to EN mass is then metered to a mixing zone where it is
- pH 5.5
13468 and EN 13472 thoroughly mixed with a blowing agent under pressure.
The mixture of thermoplastic resin and blowing agent
is then forced through a die, which imparts a shape to
the thermoplastic mass, into a zone of lower pressure
(i.e. atmospheric pressure). The blowing agent
2.4 Delivery status expands to form the cells of the foam and the product
The PE products are supplied as tubes and shaped is then cooled with water (municipal water) before
pieces. The tubes are delivered in lengths of 2 m being heat-welded to itself, due to a NMC’s proprietary
packed in cardboard. One insulation thickness of 16 technology. Finally, the product is cut to size, packed
mm is available for all common pipe diameters from and stored.
125 mm up to 200 mm inside diameter.
Quality assurance :
2.5 Base materials/Ancillary materials The manufacture is certified ISO 9001 for the quality
management.
Base materials
CLIMAFLEX® SPIRAL are flexible insulation materials
based on bio-polyethene, which is produced using a 2.7 Environment and health during
mixture of up to seven basic component materials. The manufacturing
following table displays an average weighted of During all manufacturing steps of NMC S.A. Belgium,
different elements of the formulation, and this for the the production follows all national guidelines and
complete CLIMAFLEX® SPIRAL product range. regulations. Solar panels are installed on the roof of
This LCA study was carried out on the basis of the the warehouse to reduce the requirement for grid
weighted average. electricity.
This product contains substances listed in the
candidate list (date: 08.07.2021) exceeding 0.1 Quality assurance :
percentage by mass: No. The manufacture is certified ISO 14001 -
This product contains other CMR substances in environmental management system
categories 1A or 1B, which are not on the candidate
list, exceeding 0.1 percentage by mass: No. 2.8 Product processing/Installation
Biocide products were added to this construction CLIMAFLEX® SPIRAL can be installed using basic
product or it has been treated with biocide products tools (e.g. craft knives). No special tools, nor specific
(this then concerns a treated product as defined by the protection is necessary.
(EU) Ordinance on Biocide Products No.
528/2012): No. 2.9 Packaging
CLIMAFLEX® SPIRAL products are packed in
cardboard boxes and transported on reusable pallets.
All packaging material can be recycled. The pallets
Name Value Unit
used to transport the products are taken back or
BIO-PE 69 %
exchanged when the CLIMAFLEX® SPIRAL easy is
Flame retardant 13 %
delivered, so the use of pallets is a close loop
LLDPE B 4 %
economy.
Pigment 1 Black 0,7 %
Nucleating 1.1 %
Volume stabilizer 2.6 %
Blowing Agent 9.6 % 2.10 Condition of use
BIO-PE and fillers are the main components of the During the use of the products for the purpose for
product and are responsible for the characteristics and which they are intended, there are no modifications
performance of the product unless one of the effects listed in extraordinary impacts
The blowing agent causes the expansion during occurs (see point 2.13).
manufacturing. The flame retardant ensures the fire
resistance and conformity with fire protection 2.11 Environment and health during use
regulations (see section 2.13). There are no particular effects on environmental and
According the European Chemicals Regulation health impacts during use related to the material
/REACH/ manufacturers, importers and downstream composition of the product. The CLIMAFLEX®
users must register their chemicals and are SPIRAL products are used in a wide range of
responsible for their safe use. NMC S.A. uses applications across the building sector.
exclusively verifiably registered and approved The Polyethylene Furanoate (PEF) foams fulfil the
substances in its production. Products manufactured German, Belgian and French regulations regarding the
and put on the market by NMC do need to be emission of Volatile Organic Compound (VOC) with
registered. CLIMAFLEX® SPIRAL do not contain emissions far below the most stringent limit values.
Substances of Very High Concern (SVHC). Antimony The Eurofin Product Testing institute, at the request of
trioxide and halogenated flame-retardants are applied. the CEFEP (European group of PEF and FEF
manufacturers) has made a wide range of tests for
different PEF products from different manufacturers.
2.6 Manufacture 2.12 Reference service life
The manufacturing process consists of a continuous CLIMAFLEX® SPIRAL can be used to insulate self-
extrusion. Solid pellets of thermoplastic resin are fed supporting interior ventilation pipes, as it needed no
into a melting zone in which the resin is melted, to maintenance on behalf of internal dust cleaning, the
3 Environmental Product Declaration NMC sa – CLIMAFLEX® SPIRAL
service life can be considered as being the same as CLIMAFLEX® SPIRAL is chemically inert and does not
the building life cycle. present any environmental or health risk if
mechanically destructed. CLIMAFLEX® SPIRAL is not
UV resistant. The product is not recommended for
2.13 Extraordinary effects outside applications without complementary UV
protection
Fire
According to /EN13501-1/ CLIMAFLEX® SPIRAL are 2.14 Re-use phase
classified as EURO CLASS E and therefore have a In principle, if removed carefully, CLIMAFLEX®
limited speed of inflammation. SPIRAL can be reused on any other ventilation system
of similar dimensions. Any material not suitable for
reuse is fully recyclable.
Fire protection 2.15 Disposal
Name Value CLIMAFLEX® SPIRAL is fully recyclable using the
Building material class E same recycling systems as those used for other forms
of PE waste.
Any non-recycled material should be disposed of the
Water materials according to the local regulations, and by the
CLIMAFLEX® SPIRAL is a closed cell foam and /European Waste Catalogue waste code 07 02 13
obtains the best water absorption class WS005 waste Plastic "Low Density Polyethylene"
according to the product standard
2.16 Further information
Mechanical destruction Additional information about CLIMAFLEX® SPIRAL
can be found on the NMC web site www.nmc-
insulation.com Here data sheets can be found.
3. LCA: Calculation rules
3.1 Declared Unit Module A4: Transport of the final product to the
This declaration refers to 1 m³ of produced pipe application site. The average transport distance has
insulation product. For the LCA calculations, as the been calculated based on a weighted value for NMC’s
product is foam and has some tolerances, the LCA main customers representing more than 90% of the
calculation is based on the average weight per meter sales volume in 2020. Capacity utilisation by volume is
and the density 100%. However, given the low density of the product,
The thermal conductivity coefficient (Lambda-value) capacity utilisation by mass has been estimated as
and R-value per 16 mm thickness per product brand is 10%.
provided below as additional information and support
for installers. Module A5: The products can be placed end to end
and the remaining pieces can be reused on other
Declared unit pipes. The calculations do not contain any installation
Name Value Unit waste. Cardboard as a packaging material is assumed
Declared unit 1 m3 to be recycled. As input material cardboard made of
Gross density 30 kg/m3 waste paper is considered. Thus, the environmental
conversion factor [Mass/Declared burden for packaging material is considered already in
30 -
Unit] A1-A3. The value of the environmental impact for A5 is
Volume for 1kg 0.033 m3 declared as “0”. No biogenic carbon has been
section of accounted for the recycled content of cardboard in A3
Conversion factor from 1 m³ to 1 the or A5.
Linear meter ventilation
pipe (m²) Module B1-B7:
Thermal Conductivity λ : 0.048 W/mK at (40°C) Once installed the CLIMAFLEX® SPIRAL product
R-value- thickness- : 16 mm : +/- 0,82 (m²K/W) requires no maintenance and no repair. Only manual
depending on the pipe diameter. cleaning with a brush is required to avoid a
concentration of dust into this air distribution system. It
will be dismantled by the end-of-life of the building. For
this reason, there are not expected to be any impacts
3.2 System boundary in B1 to B7 assuming correct specification and
The Data collection refers to the yearly production in installation.
2020. EPD type: cradle to gate with options (A1-A3,
A4, A5, C2, C4 and D) Module C1:
Disassembly is done manually. There are no impacts
Module A1 to A3: The LCA calculation covers the associated with C1. The information module is not
production of the raw materials, transport of these to declared.
the plant, the mixing of raw materials according to the
respective recipes, manufacturing of the foam product
and packaging for dispatch. All production takes place Module C2:
exclusively in Eynatten, Belgium. Transport at end-of-life stage is modeled as a Euro
Cargo 0-6 mix truck with diesel fuel. The average
4 Environmental Product Declaration NMC sa – CLIMAFLEX® SPIRAL
distance to either mechanical recycling, incineration or
landfills is assumed to be 100 km. 3.6 Data quality
All the foreground data requiring such energy or raw
Module C3: material coming from production, were verified and
The chosen scenario of 100% landfilling does not cross-checked before being included in the model.
require any waste processing. Module C3 is not The GaBi life cycle databases are regularly updated –
declared. in this study, the 2021 database has been used in Gabi
10 (Service Pack 2021001000) software environment.
Module C4: For electrical and Belgium energy regional specific grid
The environmental burden for the chosen scenario of mixes and Belgium specific supply for natural gas were
100% recycling is declared in module C4. considered.
The product contains raw materials from renewable
sources. By calculating the environmental burden for 3.7 Period under review
the production process the sequestration of CO from The production data for the year 2020
2
the atmosphere has been taken into account. were used for the realization of this study.
3.8 Allocation
Module D: There is no co-product or by-product generated during
The end-of-life scenarios for packaging material and the production of NMC’s products.
product do not deliver any benefits for the next system. Due to the lack of specific data per production line and
Recycling of cardboard is a closed cycle with the product, the energy has been allocated per overall
production process. produced volume of insulation foam.
The product is 100 % recycled
Production waste
3.3 Estimates and assumptions Most of the production waste from the process
The LCA calculation is conducted using the Gabi (machine start, end of production, non-conforming
ts life cycle database used in the GaBi 10 software products, etc.) is recycled in NMC Eynatten Plant.
environment (Service Pack 2021001000). . Not all These impacts are accounted for in A1-A3.
necessary LCIs are included in the database. Where
data were missing or were unavailable or where Installation and End-of-Life waste
suppliers were unable to provide complete information, Installation of the foam products is done by hand and
proxy datasets have been used. The environmental requires no special equipment apart from a knife.
burden for the production of pigments, flame retardants Installation off-cut is not considered in this calculations.
and volume stabilizers are approximated.
3.9 Comparability
3.4 Cut-off criteria Basically, a comparison or an evaluation of EPD data
Any glue and adhesive tapes used during the is only possible if all the data sets to be compared
installation (A5) have not been included as were created according to EN 15804 and the building
quantification of these materials is uncertain and their context, respectively the product-specific
use by the various installers is too diverse, eventually characteristics of performance, are taken into account.
adhesives and glues are not required in all/most cases,
but may be used for some applications.
In this study no others cut-off criteria have been
applied and all elementary incoming processes as well
as all energy and water inputs and waste outputs have
been counted.
3.5 Background data
The software system for life cycle engineering / GaBi
2021 Version 10 software environment (Service Pack
2021001000) developed by thinkstep AG was used to
perform this LCA. The GaBi LCI life cycle database
used in the GaBi 10 software environment (Service
Pack 2021001000) provides the life cycle inventory
data for several of the raw and process materials
obtained from the background system. The most
recent update of the database was in 2021.
4. LCA: Scenarios and additional technical information
transported
Transport to the building site (A4) Use or application of the installed product (B1)
Name Value Unit see section 2.12 "Use"
Litres of fuel 0.185 l/100km
Transport distance 661 km Repair (B3)
Capacity utilisation (including Name Value Unit
10 %
empty runs) Information on the repair process - -
Gross density of products 30 kg/m3 Information on the inspection process - -
5 Environmental Product Declaration NMC sa – CLIMAFLEX® SPIRAL
Number/
Repair cycle -
RSL
Water consumption - m3
Auxiliary - kg
Other resources - kg
Electricity consumption - kWh
Other energy carriers - MJ
Material loss - kg
Replacement (B4) / Refurbishment (B5)
Name Value Unit
Number/
Replacement cycle -
RSL
Electricity consumption - kWh
Litres of fuel - l/100km
Replacement of worn parts - kg
Operational energy use (B6) and Operational water
use (B7)
Name Value Unit
Water consumption - m3
Electricity consumption - kWh
Other energy carriers - MJ
Equipment output - kW
End of life (C1-C4)
Name Value Unit
Recycling 30 kg
Reuse, recovery and/or recycling potentials (D),
relevant scenario information
One of the benefits beyond the boundaries of the
system is the recyclability of the Climaflex product.
Recycled PE-LD granulate can be used as a substitute
for virgin PE-LD granulate on a one-for-one basis.
Furthermore, there are no differences in the properties
or performance of bio-based PE-LD and PE-LD
derived from fossil fuels. It is assumed that recycled
granulate generated from Climaflex products displace
the need for fossil fuel derived PE-LD granulate.
Another benefit beyond the boundaries of the system
is the recovery of energy generated from the
incineration of waste at end-of-life. This is modeled in
the GaBi7 software using an industry-average dataset
for the incineration of polyethylene and according to
the quantity of waste at end-of-life. The recovery of
thermal and electrical energy produced by the
incinerator avoids the use of fossil resources.
Name Value Unit
6 Environmental Product Declaration NMC sa – CLIMAFLEX® SPIRAL
5. LCA: Results
DESCRIPTION OF THE SYSTEM BOUNDARY (X = INCLUDED IN LCA; MND = MODULE NOT DECLARED;
MNR = MODULE NOT RELEVANT)
BENEFITS AND
CONSTRUCTI LOADS
PRODUCT STAGE ON PROCESS USE STAGE END OF LIFE STAGE BEYOND THE
STAGE SYSTEM
BOUNDARIES
7 Environmental Product Declaration NMC sa – CLIMAFLEX® SPIRAL
lairetam
waR
ylppus tropsnarT
gnirutcafunaM
eht
morf
tropsnarT
etis
eht
ot
etag
ylbmessA esU
ecnanetniaM
riapeR
tnemecalpeR tnemhsibrufeR
ygrene
lanoitarepO esu
retaw
lanoitarepO esu
noitcurtsnoc-eD
noitilomed tropsnarT
gnissecorp
etsaW
lasopsiD -esueR -yrevoceR -gnilcyceR laitnetop
A1 A2 A3 A4 A5 B1 B2 B3 B4 B5 B6 B7 C1 C2 C3 C4 D
X X X X X MND MND MNR MNR MNR MND MND MND X X X X
RESULTS OF THE LCA - ENVIRONMENTAL IMPACT according to EN 15804+A1: 1 m³
CLIMAFLEX®SPIRAL made of NMC NATUREFOAM®
Parameter Unit A1-A3 A4 A5 C2 C3 C4 D
GWP [kg CO2-Eq.] 12.48 2.07 0.00 0.18 1.94 0.00 -54.71
ODP [kg CFC11-Eq.] 1.53E-7 5.54E-16 0.00E+0 4.78E-17 1.74E-13 0.00E+0 -7.25E-13
AP [kg SO2-Eq.] 1.33E+0 1.77E-3 0.00E+0 1.53E-4 2.00E-3 0.00E+0 -6.23E-2
EP [kg (PO4)3--Eq.] 7.74E-1 3.55E-4 0.00E+0 3.06E-5 4.86E-4 0.00E+0 -9.80E-3
POCP [kg ethene-Eq.] 2.41E-1 2.30E-4 0.00E+0 1.99E-5 2.32E-4 0.00E+0 -1.11E-2
ADPE [kg Sb-Eq.] 1.02E+0 1.87E-7 0.00E+0 1.61E-8 1.44E-6 0.00E+0 -1.32E-5
ADPF [MJ] 1230.84 27.74 0.00 2.39 25.72 0.00 -2117.96
GWP = Global warming potential; ODP = Depletion potential of the stratospheric ozone layer; AP = Acidification potential of land and water; EP =
Caption Eutrophication potential; POCP = Formation potential of tropospheric ozone photochemical oxidants; ADPE = Abiotic depletion potential for non-
fossil resources; ADPF = Abiotic depletion potential for fossil resources
RESULTS OF THE LCA - INDICATORS TO DESCRIBE RESOURCE USE according to EN 15804+A1: 1 m³
CLIMAFLEX®SPIRAL made of NMC NATUREFOAM®
Parameter Unit A1-A3 A4 A5 C2 C3 C4 D
PERE [MJ] 1968.99 1.61 0.00 0.14 26.03 0.00 -133.22
PERM [MJ] 893.00 0.00 0.00 0.00 0.00 0.00 0.00
PERT [MJ] 2861.99 1.61 0.00 0.14 26.03 0.00 -133.22
PENRE [MJ] 1367.91 28.13 0.00 2.43 77.92 0.00 -2162.16
PENRM [MJ] 174.07 0.00 0.00 0.00 0.00 0.00 0.00
PENRT [MJ] 1541.98 28.13 0.00 2.43 77.92 0.00 -2162.16
SM [kg] 22.56 0.00 0.00 0.00 0.00 0.00 0.00
RSF [MJ] 0.00 0.00 0.00 0.00 0.00 0.00 0.00
NRSF [MJ] 0.00 0.00 0.00 0.00 0.00 0.00 0.00
FW [m³] 0.29 0.00 0.00 0.00 0.02 0.00 -0.24
PERE = Use of renewable primary energy excluding renewable primary energy resources used as raw materials; PERM = Use of
renewable primary energy resources used as raw materials; PERT = Total use of renewable primary energy resources; PENRE = Use of
non-renewable primary energy excluding non-renewable primary energy resources used as raw materials; PENRM = Use of non-
Caption
renewable primary energy resources used as raw materials; PENRT = Total use of non-renewable primary energy resources; SM = Use
of secondary material; RSF = Use of renewable secondary fuels; NRSF = Use of non-renewable secondary fuels; FW = Use of net fresh
water
RESULTS OF THE LCA – WASTE CATEGORIES AND OUTPUT FLOWS according to EN 15804+A1:
1 m³ CLIMAFLEX®SPIRAL made of NMC NATUREFOAM®
Parameter Unit A1-A3 A4 A5 C2 C3 C4 D
HWD [kg] 1.31E-3 1.48E-9 0.00E+0 1.28E-10 2.67E-8 0.00E+0 -3.18E-7
NHWD [kg] 1.07E+1 4.41E-3 0.00E+0 3.81E-4 8.52E-2 0.00E+0 -5.90E-1
RWD [kg] 9.44E-2 5.10E-5 0.00E+0 4.40E-6 2.06E-2 0.00E+0 -1.66E-2
CRU [kg] 0.00 0.00 0.00 0.00 0.00 0.00 0.00
MFR [kg] 0.00 0.00 22.56 0.00 30.00 0.00 0.00
MER [kg] 0.00 0.00 0.00 0.00 0.00 0.00 0.00
EEE [MJ] 0.00 0.00 0.00 0.00 0.00 0.00 0.00
EET [MJ] 0.00 0.00 0.00 0.00 0.00 0.00 0.00
HWD = Hazardous waste disposed; NHWD = Non-hazardous waste disposed; RWD = Radioactive waste disposed; CRU = Components
Caption for re-use; MFR = Materials for recycling; MER = Materials for energy recovery; EEE = Exported electrical energy; EET = Exported
thermal energy
6. LCA: Interpretation
The base polymer used at NMC is produced from of the advantages of using biopolymers is a significant
renewable raw materials (Biomass/Sugar cane). One reduction in greenhouse gas emissions compared to
the use of raw materials of fossil origin. In addition, the of raw materials and their transport account for almost
use of non-renewable raw materials is avoided in this 80% of the impact Global Warming Potential.
way. When we analyse the complete life cycle we see One way to continue to reduce the environmental
that the most impacting part for all environmental impact of the CLIMAFLEX® SPIRAL would be to
impact factors is the production module and more continue to diversify our energy sources by switching
particularly the raw materials. With regard to global more and more to renewable energies. To this end,
warming for the complete life cycle, more than 83% after having greatly increased the number of
comes from the production module 2.1% of transport to photovoltaic panels, NMC will acquire a cogeneration
the places of installation and 14.3% comes from the system. Looking for more eco-responsible suppliers
end of life. For all other impact factors, more than 90% must also be put in place, as well as finding raw
of the impacts come from the production phase. materials manufactured locally to avoid long-distance
Transport has a more pronounced impact on global transport as much as possible.
warming potential as well as on soil and water An analysis of the plant's carbon footprint, which is
acidification potential and abiotic fossil resource currently being carried out, should enable NMC to
depletion potential. A more in-depth analysis of the identify areas for improvement and find solutions to
production module A1 to A3 shows that the production achieve the goal of zero carbon.
7. Requisite evidence
7.1. VOC emissions Sum SVOC (C16 - C22) - μg/m3
Eurofins Product Testing A/S has tested a wide range R (dimensionless) - -
and variety of typical PEF (Polyethylene Furanoate VOC without NIK - μg/m3
foam) products marketed in the EU from CEFEP Carcinogenic Substances - μg/m3
(European Group of PEF/FEF manufacturers) Based
on the loading factor 0.05m²/m3 (determined after AgBB overview of results (3 days [µg/m³])
consideration of the real life applications of PEF Name Value Unit
products (in living rooms) and recommendations by the TVOC (C6 - C16) - μg/m3
experts of the test institute) all results were found to be Sum SVOC (C16 - C22) - μg/m3
clearly below the limit values. For all samples below
R (dimensionless) - -
100mg/m3 TVOC after 28 days. Certificates are
VOC without NIK - μg/m3
available on request.
Carcinogenic Substances - μg/m3
7.2 Leaching
VOC Emissions
According to /EN 13468/ the content of water-soluble
Name Value Unit
chloride ions for CLIMAFLEX® is <15mg/kg
Overview of Results (28 Tage) - μg/m3
TVOC (C6 - C16) - μg/m3
8. References
EN 1602 ISO 14040: Environmental management — Life cycle
EN 1602: 2013: Thermal insulating products for assessment — Principles and framework
building applications - Determination of the apparent
density ISO 14044
ISO 14044: Environmental management — Life cycle
EN ISO 8497 assessment — Requirements and guidelines
EN ISO 8497: Thermal insulation - Determination of
steady-state thermal transmission properties of thermal EN 14707
insulation for circular pipes EN 14707: 2012: Thermal insulating products for
building equipment and industrial installations.
ISO 9001 Determination of maximum service temperature for
ISO 9001: 2015: Quality management systems. preformed pipe insulation
EN 13501-1 EN 15804
EN 13501-1:2007+A1: 2013 Fire classification of EN 15804: 2012-04 + A1 2014: Sustainability of
construction products and building elements - construction works — Environmental Product
Classification using test data from reaction to fire tests Declarations — Core rules for the product category of
construction products
ISO 14001
ISO 14001: 2015 Environmental management CEN/TR 15941
systems. CEN/TR 15941: Sustainability of construction works -
Environmental product declarations - Methodology for
EN ISO 14025 selection and use of generic data
EN ISO 14025: 2011-10: Environmental labels and
declarations — Type III environmental declarations — CEN TS 16516
Principles and procedures CEN TS 16516: /AgBB/, /ISO 16000-3/, /ISO 16000-6/,
/ISO16000-9/, /ISO 16000-11/ Construction products -
ISO 14040 Assessment of release of dangerous substances.
Determination of emissions into indoor air
8 Environmental Product Declaration NMC sa – CLIMAFLEX® SPIRAL
EN 16783 Product Category Rules for Building-Related
EN 16783: 2017 Thermal insulation products - Product Products and Services
category rules (PCR) for factory made and in-situ Institute Construction and Environment e.V. (IBU)
formed products for preparing environmental product Part A: Calculation Rules for the Life Cycle
declarations Assessment and Requirements on the Project Report
Version 1.7
Eurostat
European Statistics: Recovery rates for packaging PCR Guidance-Texts for Building-Related Products
waste Paper and cardboard packaging for the and Services
European Union 27 countries 2014 From the range of Environmental Product Declarations
http://ec.europa.eu/eurostat/home of Institute Construction and Environment e.V. (IBU)
Part B: Requirements on the EPD for Insulating
Eurofins materials made of foam plastics
Eurofins: Product Testing Institute Version 1.6 (Template) Version 1.2 (PCR specific)
Gabi ts Sphera
GaBi 10 GaBi Software-System and Database for Life Sphera Solutions Gmbh. GaBi 10 LCI documentation.
Cycle Engineering Copyright © 1992-2021 Sphera GaBi Databases (sphera.com) Stuttgart,
Solutions Gmbh Version: 10.5.0.78 DB Schema 8007 Echterdingen: Sphera Solutions Gmbh
Institut Bauen und Umwelt
Institut Bauen und Umwelt e.V., Berlin(pub.): General
Instructions for the EPD Programme of Institut Bauen
und Umwelt e.V., Version 2.0 2021
9 Environmental Product Declaration NMC sa – CLIMAFLEX® SPIRAL
Publisher
Institut Bauen und Umwelt e.V. Tel +49 (0)30 3087748- 0
Panoramastr. 1 Fax +49 (0)30 3087748- 29
10178 Berlin Mail info@ibu-epd.com
Germany Web www.ibu-epd.com
Programme holder
Institut Bauen und Umwelt e.V. Tel +49 (0)30 - 3087748- 0
Panoramastr 1 Fax +49 (0)30 – 3087748 - 29
10178 Berlin Mail info@ibu-epd.com
Germany Web www.ibu-epd.com
Author of the Life Cycle
Assessment Tel +32 (0) 87 85 85 00
NMC S.A. Fax +32 (0) 87 85 85 11
Gerd-Noël-Strasse 1 Mail info@nmc.eu
4731 Eynatten Web www.nmc.eu
Belgium
Owner of the Declaration
NMC S.A. Tel +32 (0) 87 85 85 00
Gerd-Noël-Strasse 1 Fax +32 (0) 87 85 85 11
4731 Eynatten Mail info@nmc.eu
Belgium Web https://nmc-insulation.com/
