ENVIRONMENTAL PRODUCT DECLARATION
as per ISO 14025 and EN 15804+A2
Owner of the Declaration Aggregate Industries
Programme holder Institut Bauen und Umwelt e.V. (IBU)
Publisher Institut Bauen und Umwelt e.V. (IBU)
Declaration number IBU-CEI-HOL-2205120-UK2023000437-1SUE001-EN
Issue date 19/10/2023
Valid to 18/10/2028
Concrete C60/75 Dynamax CIIIA produced in plant Bow
Mix code BWL2922/018, EPD Version 1
Aggregate Industries
www.ibu-epd.com | https://epd-online.com
1. General Information
Aggregate Industries C60/75 Dynamax CIIIA
Programme holder Owner of the declaration
IBU - Institut Bauen und Umwelt e.V. Aggregate Industries
Hegelplatz 1 Bardon Hall
10117 Berlin LE67 1TL Coalville
Germany United Kingdom
Declaration number Declared product / Declared unit
IBU-CEI-HOL-2205120-UK2023000437-1SUE001-EN 1 m3 of unreinforced concrete C60/75 Dynamax
CIIIA
This declaration is based on the product Scope:
category rules: This document refers to the production of
Concrete components made of in-situ or ready- C60/75 Dynamax CIIIA concrete, mix code
mixed concrete, 03.2022 (PCR checked and BWL2922/018 produced in the plant of Bow of
approved by the SVR) Aggregate Industries in United Kingdom for use
as concrete in building construction and civil
Issue date engineering.
19/10/2023
The EPD was calculated with the pre-verified
Valid to software CarbonCLARITYTM EN 15804 EPD
18/10/2028 Generator - RMX of Climate Earth.
The owner of the declaration shall be liable for
the underlying information and evidence; the
IBU shall not be liable with respect to
manufacturer information, life cycle assessment
data and evidences.
The EPD was created according to the
specifications of EN 15804+A2. In the following,
the standard is simply referred to as EN 15804.
Verification
The standard EN 15804 serves as the core PCR
Independent verification of the declaration and data
according to ISO 14025:2011
Hans Peters internally x externally
(Chairman Institut Bauen und Umwelt e.V.)
Florian Pronold Matthias Schulz
(Managing Director Institut Bauen und Umwelt e.V.) (Independent verifier)
3 EPD Aggregate Industries – BWL2922/018 concrete, Plant Bow
2. Product
2.1 Product description/Product definition 2.5 Base materials/Ancillary materials
Concrete is produced by mixing cement, aggregates Name Value Unit
and water with potentially additional cementitious Cement ca. 10-17 M.%
materials, fibers and additives.
Water ca. 4-7 M.%
Aggregate ca. 70-90 M.%
The fresh concrete is generally poured into formwork,
compacted and hardened in the desired form by Cementitious ca. 7-10 M.%
hydration of the cement to form a solid artificial rock. Fibers ca. <1 M.%
Admixtures ca. <1 M.%
The declared product is unreinforced concrete that is
delivered to the job site as ready-mix concrete. In the
case of reinforced components, the proportion of
reinforcing steel must be taken into account
separately.
To calculate the life cycle assessment of the C60/75
Dynamax CIIIA concrete in plant Bow, the production
data from mix code BWL2922/018 were used.
For the use and application of the product the
respective national provisions at the place of use
apply, such as the building codes and the
corresponding national specifications.
Note: dashed lines indicate production steps that do not
2.2 Application necessarily apply to this concrete
Concrete is a widely used building material in the
construction industry. It is used for example for the This product contains substances listed in the ECHA
construction of walls, stairs, floor, foundations, bored candidate list (date: 19.05.2022) exceeding 0,1
piles or even complete structures such as bridges. percentage by mass: no
2.3 Technical data This product contains other CMR substances in
Concrete C60/75 Dynamax CIIIA has the following categories 1A or 1B which are not on the candidate
technical properties: list, exceeding 0,1 percentage by mass: no
Technical data Biocide products were added to this construction
Name Value Unit product or it has been treated with biocide products
Gross density 2416 kg/m3 (this then concerns a treated product as defined by the
(EU) Ordinance on Biocide Products No. 528/2012): no
Compressive
C60/75 N/mm2
strength
2.6 Manufacture
The dosed aggregates are first premixed with cement
This concrete product is produced according to as a binding agent and other additives. The mixture is
standard BS 8500:2019 Concrete - Complementary then mixed with water to form a plastically deformable
British Standard to BS EN 206 as a designed concrete. fresh concrete. This is transported to the customer
where it is placed in the prepared formwork and
This technical data fulfill the requirements according to compacted.
BS 8500 standard regarding quality control and
conformity checks. Testing is done according to EN To ensure the quality of the concrete, quality
12350 and EN 12390. Further technical data, as assurance systems is installed in Bow plant, which is
indicated in PCR B, are not relevant for this product. based on the requirements for in-house production
This is because properties such as thermal control in BS 8500 standard.
conductivity, tensile strength or modulus of elasticity
can be found in the regulations for the design of 2.7 Environment and health during manufacturing
concrete components and are therefore not routinely Fresh concrete and residual water recycling is
checked. common practice in the Bow plant. Not yet hardened
concrete residues from mixers, concrete vehicles,
Performance characteristics for fresh concrete in bucket conveyors and concrete distributors are
relation to its characteristics according to the relevant washed out and both the aggregate and the remaining
technical regulation (no CE marking). water are reused as concrete raw materials.
2.4 Delivery status Fresh concrete contains a strongly alkaline solution
Fresh concrete is delivered to the customers in that is created when cement is mixed with water and
concrete truck mixers. It can also be picked up by the can cause skin and eye irritation. The abrasiveness of
client using their trucks. the aggregate used can also support this irritation.
4 EPD Aggregate Industries – BWL2922/018 concrete, Plant Bow
Cements used within this product are low in chromate, flammable". In the event of fire, no toxic gases and
as per requirements of REACH regulation, in order to vapors can arise, and burning concrete components do
limit the development of allergic chromate dermatitis not drip or fall off.
that can happen in the event of prolonged contact with
the concrete. High fire resistance classes can be achieved through
appropriate dimensioning of the components (in EN
Further information can be found in the safety data 1992-1-2 tabular values for fire resistance classes
sheets. according to EN 13501-2 are given).
https://www.aggregate.com/news-and-resources/
technical-information/safety-data-sheets Fire protection
Name Value
2.8 Product processing/Installation Building material class A1 "not combustible"
In general, after mixing the concrete is transported to
the construction site with trucks, placed in the prepared
Water
formwork by direct pouring or pumping and usually
When exposed to water (e.g. floods), concrete is
compacted with internal vibrators. After a sufficiently
largely inert. No substances are washed out in
long hardening time, the formwork is removed and the
quantities that could be hazardous to water.
concrete is cured further with time.
Mechanical destruction
2.9 Packaging
The mechanical destruction of concrete, e.g. by
The delivery of concrete does not require the use of
demolishing concrete, does not produce any
packaging material.
substances that are hazardous to the environment or
health.
2.10 Condition of use
The composition of the concrete does not
2.14 Re-use phase
fundamentally change when it is used.
Components made of concrete can be dismantled. The
concrete is first crushed and separated into individual
2.11 Environment and health during use
grain fractions and used in road construction or in
The natural ionizing radiation from concrete is low and
small proportions as recycled aggregate for the
harmless to health. The environmental compatibility of
production of fresh concrete. If steel fibers or rebar is
concrete is ensured by the fact that only standardized
included in the concrete, this is separated during or
starting materials may be used that are a priori
after demolition and reused as scrap. Recovery of
regarded as harmless.
alternative fibers or rebar is not commonplace.
2.12 Reference service life
2.15 Disposal
A reference service of 50 years is used for modeling
For construction waste made of concrete, the waste
concrete’s use phase.
codes 17 01 01 (concrete), 17 04 05 (steel fibers) and
17 02 13 (plastic fibers) (WCO) apply in accordance
2.13 Extraordinary effects
with the European list of waste.
Fire
2.16 Further information
According to EN 13501-1, concrete meets the
Further information www.aggregate.com.
requirements of building material class A1, "non-
5 EPD Aggregate Industries – BWL2922/018 concrete, Plant Bow
3. LCA: Calculation rules
3.1 Declared unit
1 m3 of unreinforced concrete C60/75 Dynamax CIIIA End of life
In the case of reinforced components, the proportion of Module C1: Dismantling /
reinforcing steel must be taken into account demolition of concrete buildings /
separately. components
Declared unit Module C2: Transport of
Designation Value unit demolished concrete for processing
Declared unit 1 m3
Module C3: Concrete waste
Density 2416 kg/m3
processing
Conversion factor to 1 kg 4.14E-4 -
Module D
To calculate the life cycle assessment of the C60/75
Dynamax CIIIA concrete in plant Bow, the production Module D: Benefits and loads for
data from mix code BWL2922/018 were used. the use of concrete demolition
waste as replacement for primary
3.2 System boundary materials
Type of EPD: cradle to gate with options, modules
C1–C4, and module D (A1–A3 + C + D and additional 3.3 Estimates and assumptions
modules A4, A5 and B1) No estimates or assumptions were made that would be
relevant for the interpretation of the life cycle
The selected system boundaries include the assessment results.
production of the concrete including the extraction of
raw materials through to the installation, use and end 3.4 Cut-off criteria
of life of the finished product. All raw materials for the production of concrete, all
transport as well as all energy and water consumption
Material production and placement for production, mixing, placing and waste treatment of
the concrete were taken into account.
Module A1: Extraction and
processing of the raw materials The environmental impacts from the production and
used in concrete production use of the formwork were neglected for the life cycle
assessment of the concrete production. With the usual
Module A2: Transport of the raw frequency of use of formwork, the mass of resources
materials to the plant and primary energy used is less than 1% of the total
values for concrete production. The materials used for
Module A3: Concrete production in concrete curing were also excluded as they represent
the plant and waste treatment less than 1% of the total mass and primary energy use
for concrete production.
Module A4: Transport to the 3.5 Background data
construction site The CarbonCLARITYTM EN 15804 EPD Generator -
RMX version 1.0.0 dated 01/08/2023 with configuration
Module A5: Includes all file dated 19/10/2023 was used for the life cycle
processes associated with placing assessment.
the concrete (e.g. pumping or
installation by crane) as well as the Datasets from EPDs and from the Ecoinvent database
production, transport and treatment (version 3.8) were used for the calculation.
of unused concrete (e.g. return
concrete) 3.6 Data quality
The data basis for this EPD is the continuous data
Use phase acquisition in the Bow plant. The data collected were
reviewed for plausibility by Climate Earth and were
Module B1: Carbonation during the rated as very good quality.
use phase
The background datasets are on average less than 5
Module B2-B7: For concrete years old and their quality is rated as good or very
components, maintenance, repair good.
refurbishment or replacement
measures are not usually required 3.7 Period under review
during the reference service life. For the life cycle assessment of the C60/75 Dynamax
Therefore, no environmental CIIIA, data from the period 01/07/2021 to 30/06/2022
burden is considered in these were used.
modules.
6 EPD Aggregate Industries – BWL2922/018 concrete, Plant Bow
3.8 Geographic Representativeness The alternative fuels used for production are classified
Land or region, in which the declared product system as either secondary fuels or waste. Emissions from
is manufactured, used or handled at the end of the secondary fuels are included in the environmental
product´s lifespan: United Kingdom impact assessment results, while emissions from the
incineration of waste are reported as additional.
3.9 Allocation
Cementitious products such as fly ash, blast furnace Energy and auxiliary materials used in the production
slag or silica fume are considered co-products and of concrete are allocated to each individual concrete
economic allocation is used. mix based on the total volume of concrete produced in
the plant.
The alternative fuels used for the production of the
cements used are classified either as secondary fuels Finally, the use of recycled and/or secondary raw
or as waste. Emissions from secondary fuels are materials is allocated to each individual concrete mix
included in the impact assessment results while based on their actual composition.
emissions from waste fuels are reported as additional
information according to the IBU Cement PCR. The 3.10 Comparability
waste status of the fuels concerned was verified using Basically, a comparison or an evaluation of EPD data
their waste codes. The exclusion of the impact due to is only possible if all the data sets to be compared
the combustion of combustible waste was only applied were created according to EN 15804 and the building
to CO2 emissions, as other emissions (eg, NOx, SOx, context, respectively the product-specific
etc.) were not easily differentiated from the different characteristics of performance, are taken into account.
types of fuels.
The Ecoinvent background database is used (version
3.8).
7 EPD Aggregate Industries – BWL2922/018 concrete, Plant Bow
4. LCA: Scenarios and additional technical information
Information on describing the biogenic Carbon where
Content at factory gate
Name Value Unit k = k-factor sourced from EN 16757 standard
Biogenic Carbon Content in depending on structure type, exposure condition
0 kg C
product and concrete strength class [mm/year0,5]
Biogenic Carbon Content in t = service life (yr)
0 kg C
accompanying packaging A = area of concrete element (m2/m3)
i
D = degree of carbonation sourced from EN 16757
c
Note: 1 kg biogenic Carbon is equivalent to 44/12 kg standard depending on structure type and exposure
of CO condition (%)
2
C = 159 (kg CO/m3). It is calculated as per EN
factor 2
Module A4: Transport to jobsite 16757 standard based on the concrete
The following table shows the data used in the composition
modelling of product transport to the jobsite:
Module B2-B7:
Transport to the building site (A4) No maintenance or repair is usually required for
Name Value Unit concrete during its reference service life. In addition,
lt diesel no energy or water are consumed during its use.
Litres of fuel (per m3 concrete) 4.60 eq./100
km* Module C1-C4:
Transport distance 5.57 km According to the current state of the art, structures
Capacity utilization (including made of concrete and reinforced concrete are mainly
45.6 %
empty runs) dismantled with long-front excavators equipped with
Gross density of products demolition claws.
2416 kg/m3
transported
Capacity utilization volume Name Value Unit
factor 0.91 - Diesel consumption for 2.9 lt/m3
demolition process
* If trucks are not powered by diesel, the necessary energy
consumption is converted into the equivalent diesel Demolition waste collected 2416 kg
consumption. Therefore the total fuel consumption can be
expressed in a single unit of liters of diesel equivalent / 100 The demolished concrete material is then transported
km. to the crushing plant according to the following details.
Module A5: Installation of concrete
Name Value Unit
The following table shows the data used in the
Truck 25 km
modelling of product installation:
The processing of concrete rubble is usually carried
Installation into the building (A5)
out using jaw or impact crushers, which, in addition to
Name Value Unit
pure breaking, also perform a pre-screening and metal
Electricity consumption 0.25 kWh
separation.
Other energy carriers 18.4 MJ
Material loss 38.4 kg In United Kingdom 97% of concrete waste is recycled
or used for backfilling while less than 3% ends up in
Module B1: Carbonation landfills (DEFRA).
Through carbonation, concrete components absorb
carbon dioxide from the air during their useful life. This Therefore, one scenario for 100% recycling is
can be expressed as a negative global warming considered in this life cycle assessment.
potential in module B1 and is calculated according to
EN 16757 using the following data. Name Value Unit
For reuse 0 kg
Carbonation during use For recycling 2416 kg
Name Value Unit
For landfill 0 kg
Structure type Building -
Building,
The carbonation of concrete rubble during the end of
Exposure condition exterior, -
life phase is modelled according to the guidelines of
exposed to rain
EN 16757 standard.
Service life 50 yr
Area to volume ratio 5 m2/m3 Module D: Benefits and loads beyond the system
Weight per unit area 483 kg/m2 boundary
The output at the end of the crushing process can
Carbonation results for alternative scenarios can be replace the primary materials sand / gravel and
calculated using the following formula crushed stone as secondary material. Potentially
recovered steel fibers can be used for the production
k∗√t of new steel products.
CO uptake= ∗A ∗D ∗C
2 1000 i c factor
The net output flow calculation in Module D considers
secondary material input flows from aggregates and
8 EPD Aggregate Industries – BWL2922/018 concrete, Plant Bow
fibers while excluding small secondary material inputs The credits in the LCA results for the replacement of
from other raw materials such as cement, cementitious primary raw materials are shown in module D.
or admixtures. Additional output flows from the A5 life
cycle stage are also excluded.
9 EPD Aggregate Industries – BWL2922/018 concrete, Plant Bow
5. LCA: Results
The table below contains the life cycle assessment results for a declared unit of 1 m3 of unreinforced concrete
C60/75 Dynamax CIIIA.
The characterization factors of the "Environmental Footprint reference Package 3.0" were used to determine the
LCA results.
DESCRIPTION OF THE SYSTEM BOUNDARY (X = INCLUDED IN LCA; ND = MODULE OR INDICATOR NOT
DECLARED; MNR = MODULE NOT RELEVANT)
BENEFITS AND
CONSTRUCTI LOADS
PRODUCT STAGE ON PROCESS USE STAGE END OF LIFE STAGE BEYOND THE
STAGE SYSTEM
BOUNDARIES
ylppus
lairetam
waR
tropsnarT
gnirutcafunaM
etag
eht
morf
tropsnarT
etis
eht
ot
ylbmessA esU
ecnanetniaM
riapeR
tnemecalpeR tnemhsibrufeR
esu
ygrene
lanoitarepO
esu
retaw
lanoitarepO
noitcurtsnoc-eD
noitilomed tropsnarT
gnissecorp
etsaW
lasopsiD -esueR -yrevoceR -gnilcyceR laitnetop
A1 A2 A3 A4 A5 B1 B2 B3 B4 B5 B6 B7 C1 C2 C3 C4 D
x x x x x x ND MNR MNR MNR ND ND x x x ND x
RESULTS OF THE LCA - ENVIRONMENTAL IMPACT according to EN 15804+A2: 1 m3
Core Indicator Unit A1-A3 A4 A5 B1 C1 C2 C3 D
GWP-total [kg CO2-Eq.] 284 1.63 6.39 -5.24 9.00 4.44 1.72 -4.32
GWP-fossil [kg CO2-Eq.] 282 1.63 6.37 -5.24 9.00 4.44 1.72 -4.32
GWP-biogenic [kg CO2-Eq.] 1.75 2.1E-4 0.03 0 7.31E-4 3.47E-4 7.87E-4 -5.01E-3
GWP-luluc [kg CO2-Eq.] 0.03 2.5E-5 6E-4 0 2.22E-4 8.01E-5 1.68E-4 -2.83E-4
ODP [kg CFC11-Eq.] 5.36E-6 3.85E-7 4.83E-7 0 2.02E-6 9.82E-7 5.83E-7 -7.3E-7
AP [mol H+-Eq.] 0.57 4.05E-3 0.03 0 0.10 0.02 0.02 -0.03
EP-freshwater [kg P-Eq.] 0.02 1.21E-5 3.44E-4 0 5.4E-5 8.2E-5 1.21E-3 -7.32E-4
EP-marine [kg N-Eq.] 0.15 1.29E-3 0.01 0 0.04 4.74E-3 0.01 -0.01
EP-terrestrial [mol N-Eq.] 1.67 1E-2 0.11 0 0.48 0.05 0.11 -0.15
POCP [kg NMVOC-Eq.] 0.45 2.01E-3 0.03 0 0.11 0.01 0.03 -0.04
ADPE [kg Sb-Eq.] 6.52E-6 1.06E-7 2.01E-7 0 4.66E-7 3.6E-7 1.91E-7 -9.62E-7
ADPF [MJ] 1643 23.0 53.4 0 125 61.4 81.0 -71.2
WDP [m³ world-Eq deprived] 21.2 1.19E-3 0.35 0 0.03 0.02 0.05 -8.50
GWP = Global warming potential; ODP = Depletion potential of the stratospheric ozone layer; AP = Acidification potential of land and
water; EP = Eutrophication potential; POCP = Formation potential of tropospheric ozone photochemical oxidants; ADPE = Abiotic
Legend
depletion potential for non fossil resources; ADPF = Abiotic depletion potential for fossil resources; WDP = Water (user) deprivation
potential
RESULTS OF THE LCA - INDICATORS TO DESCRIBE RESOURCE USE according to EN 15804+A2: 1 m3
Indicator Unit A1-A3 A4 A5 B1 C1 C2 C3 D
PERE [MJ] 322 0.73 5.30 0 0.20 0.08 2.17 -2.66
PERM [MJ] 0.34 0 5.34E-3 0 0 0 0 0
PERT [MJ] 322 0.73 5.30 0 0.20 0.08 2.17 -2.66
PENRE [MJ] 1626 23.0 53.1 0 125 61.4 81.0 -71.2
PENRM [MJ] 24.7 0 0.39 0 0 0 0 0
PENRT [MJ] 1651 23.0 53.5 0 125 61.4 81.0 -71.2
SM [kg] 37.5 0 0.60 0 0 0 0 2416
RSF [MJ] 258 0 4.09 0 0 0 0 0
NRSF [MJ] 660 0 10.5 0 0 0 0 0
FW [m³] 4.55 1.1E-3 0.07 0 1.67E-3 8.44E-4 8.52E-3 -3.12
PERE = Use of renewable primary energy excluding renewable primary energy resources used as raw materials; PERM = Use
of renewable primary energy resources used as raw materials; PERT = Total use of renewable primary energy resources;
PENRE = Use of non-renewable primary energy excluding nonrenewable primary energy resources used as raw materials;
Legend
PENRM = Use of non-renewable primary energy resources used as raw materials; PENRT = Total use of non-renewable
primary energy resources; SM = Use of secondary material; RSF = Use of renewable secondary fuels; NRSF = Use of non-
renewable secondary fuels; FW = Use of net freshwater
10 EPD Aggregate Industries – BWL2922/018 concrete, Plant Bow
RESULTS OF THE LCA – WASTE CATEGORIES AND OUTPUT FLOWS according to EN 15804+A2: 1 m3
Indicator Unit A1-A3 A4 A5 B1 C1 C2 C3 D
HWD [kg] 0.52 3.27E-3 0.01 0 7.09E-3 0.01 0.01 -0.03
NHWD [kg] 17.0 0.01 0.29 0 0.08 0.06 0.06 -0.15
RWD [kg] 0.04 1.64E-4 8.78E-4 0 8.91E-4 4.33E-4 6.07E-4 -5.17E-4
CRU [kg] 0 0 0 0 0 0 0 0
MFR [kg] 0.02 0 38.4 0 0 0 2416 0
MER [kg] 0 0 0 0 0 0 0 0
EEE [MJ] 0 0 0 0 0 0 0 0
EET [MJ] 0 0 0 0 0 0 0 0
HWD = Hazardous waste disposed; NHWD = Nonhazardous waste disposed; RWD = Radioactive waste disposed; CRU =
Legend Components for reuse; MFR = Materials for recycling; MER = Materials for energy recovery; EEE = Exported electrical energy;
EEE = Exported thermal energy
RESULTS OF THE LCA – additional impact categories according to EN 15804+A2: 1 m3
Indicator Unit A1-A3 A4 A5 B1 C1 C2 C3 D
PM [Disease Incidence] 4E-6 1.06E-7 5.46E-7 0 2.61E-6 3.73E-7 5.56E-7 -8.3E-7
IRP [kBq U235-Eq.] 17.6 0.10 0.48 0 0.55 0.27 1.74 -1.08
ETP-fw [CTUe] 727 10.4 20.1 0 41.5 29.5 15.7 -22.5
HTP-c [CTUh] 1.5E-7 1.6E-10 2.5E-9 0 5.42E-10 3.98E-10 2.19E-10 -7.98E-10
HTP-nc [CTUh] 3.15E-6 1.81E-8 5.91E-8 0 4.25E-8 5.31E-8 1.34E-8 -2.39E-8
SQP [-] 925 11.7 16.0 0 0.79 0.53 16.4 -258
PM = Potential incidence of disease due to PM emissions; IRP = Potential Human exposure efficiency relative to U235;
Legend ETPfw = Potential comparative Toxic Unit for ecosystems; HTPc = Potential comparative Toxic Unit for humans
(cancerogenic); HTPnc = Potential comparative Toxic Unit for humans (not cancerogenic); SQP = Potential soil quality index
nuclear fuel cycle. It does not consider effects due
On Global Warming Potential (GWP): to possible nuclear accidents, occupational
Net values are declared for all GWP indicators in A1 exposure nor radioactive waste disposal in
– A3. The waste status of the (waste-based) fuels underground facilities. Potential ionizing radiation
used in cement production has been verified. Gross from the soil, radon and from some construction
emissions (i.e. including CO from incineration of materials is also not measured by this indicator.
2
waste) are 340 kg CO-eq. / t (GWP-total), 338 kg
2
CO-eq. / t (GWP fossil), 1.75 kg CO eq. / t (GWP-
2 2 Disclaimer 2 –for the indicators: “abiotic depletion
biogenic).
potential for fossil resources”, “abiotic depletion
potential for non-fossil resources”, “water (user)
For wastes with biogenic carbon content, gross CO deprivation potential”, “deprivation-weighted water
2
emissions correspond to the uptake of biogenic consumption”, “potential comparative toxic unit for
CO2 during the biomass growth phase. ecosystems”, “potential comparative toxic unit for
humans - cancer effects”, “potential comparative
toxic unit for humans – non-cancer effects”,
Disclaimer 1 – for the indicator “potential Human
“potential soil quality index”. The results of this
exposure efficiency relative to U235“. This impact
environmental impact indicator shall be used with
category deals mainly with the eventual impact of
care as the uncertainties on these results are high
low dose ionizing radiation on human health of the
or as there is limited experience with the indicator.
11 EPD Aggregate Industries – BWL2922/018 concrete, Plant Bow
6. LCA: Interpretation
The following tablet shows the most important influencing factors on important indicators of the impact and life
cycle inventory analysis.
Category GWP AP EP POCP PERT PENRT ADPE FW PM
total terrestrial
Cement 71.8 % 40.0 % 49.3 % 44.6 % 10.5 % 41.5 % 59.6 % 4.49 % 35.1 %
Aggregate 1.59 % 4.83 % 7.78 % 7.00 % 1.05 % 4.89 % 12.0 % 53.8 % 17.4 %
Cementitious 19.2 % 41.4 % 28.0 % 34.4 % 83.3 % 28.6 % 10.0 % 36.6 % 36.9 %
Fibers 0 % 0 % 0 % 0 % 0 % 0 % 0 % 0 % 0 %
Admixtures 1.55 % 1.01 % 1.02 % 1.06 % 1.96 % 4.95 % 6.73 % 0.35 % 0 %
Other materials
and processes 5.86 % 12.8 % 13.9 % 12.9 % 3.19 % 20.1 % 11.6 % 4.70 % 10.6 %
Total 100% 100% 100% 100% 100% 100% 100% 100% 100%
Cement: Includes the impacts for the production of all cements used. Aggregate: Includes the impacts for the production
of sand and gravel. Cementitious: Includes the impacts for the production of all cementitious materials used such as
Legend slag, fly ash or limestone. Fibers: Includes the impacts for the production of fibers. Admixtures: Includes the impacts for
the production of concrete admixtures such as plasticisers or retarders. Other materials and processes: Includes the
impacts of materials or production processes not covered by the above categories.
In the production of concrete, cement production materials. The contribution of other processes in the
dominates all impact categories. This applies in plant is low, especially with regard to greenhouse,
particular to the global warming potential (GWP). acidification and eutrophication impact categories.
Another major influencing factor is the
extraction/production and transport of the raw
7. Requisite evidence
7.1 Radioactivity concentrations will equate to an annual effective dose
Measurements of the specific activity (gamma of about 0.25 mSv (excess to the dose received
spectrometry) in Europe resulted in the following outdoors) (Radiation Protection 112).
typical values for concrete (Radiation Protection 112)
(in Bq/kg concrete). In United Kingdom there are currently no statutory limit
values for assessing the radioactivity of building
Element Typical values (max values) materials.
RA226 40 (240)
7.2 VOC emissions and leaching
Th228 30 (190)
The environmental compatibility of concrete is ensured
K40 400 (1600)
by the fact that only standardized starting materials
may be used that are a priori regarded as harmless.
Radiation exposure in an apartment block made of Therefore, no tests are normally carried out for VOC
concrete with the above average activity emissions and leaching of concrete.
8. References
Standards BS EN 16757:2017. Sustainability of construction
works. Environmental product declarations. Product
EN 12350 Category Rules for concrete and concrete elements
BS EN 12350-4:2019 Testing fresh concrete
EN 1992-1-2
EN 12390 BS EN 1992-1-2:2004+A1:2019, Eurocode 2. Design
BS EN 12390-3:2019 Testing hardened concrete of concrete structures - General rules. Structural fire
design
EN 13501-1
BS EN 13501-1:2018, Fire classification of EN ISO 14025
construction products and building elements - BS EN ISO 14025:2011, Environmental labels and
Classification using data from reaction to fire tests declarations. Type III environmental declarations.
Principles and procedures
EN 13501-2
BS EN 13501-2:2016 Fire classification of construction EN 15804
products and building elements. Classification using EN 15804:2012+A2+AC:2021, Sustainability of
data from fire resistance tests, excluding ventilation construction works. Environmental product
services declarations. Core rules for the product category of
construction products
EN 16757
12 EPD Aggregate Industries – BWL2922/018 concrete, Plant Bow
BS 8500 concerning the making available on the market and
BS 8500:2019 Concrete - Complementary British use of biocidal products
Standard to BS EN 206
Radiation Protection 112
Other literature European Commission, Directorate-General for
Environment, Radiological protection principles
CarbonCLARITYTM EN 15804 EPD Generator - RMX concerning the natural radioactivity of building
Version 1.0.0 dated 01/08/2023 materials, Publications Office, 2000
www.climateearth.com
REACH Regulation
ECHA Registration, Evaluation, Authorisation and Restriction
European Chemicals Agency (ECHA): Candidate List of Chemicals, EG 1907/2006:2006-12-18
of Substances of Very High Concern for Authorization.
https://echa.europa.eu/ WCO
Waste Catalog Ordinance (WCO), December 10th
DEFRA 2001
Department for Environment Food & Rural Affairs
(DEFRA), UK statistics on waste, May 2022: PCR Part A
Department for Environment Food & Rural Affairs Product category rules for building related products
(DEFRA), UK statistics on waste, May 2022 and services. Part A: Calculation rules for the life cycle
assessment and requirements for the project report
Ecoinvent according to EN 15804+A2:2021 (v1.2). Berlin: Institut
Database, version 3.8, Ecoinvent, 2021. Bauen und Umwelt e.V., 17/11/2021
EF 3.0 PCR Cement
Environmental Footprint, ref package 3.0, November Product category rules for building related products
2019 (European Platform on Life Cycle Assessment and services. Part B: Requirements for the EPD for
(EPLCA)) cement, version 1.7. Berlin: Institut Bauen und Umwelt
e.V. (ed.), 05/05/2022.
IBU 2021 www.ibu-epd.com
Institut Bauen und Umwelt e.V.: General instructions
for the EPD program of Institut Bauen und Umwelt e.V. PCR Part B
Version 2.0, Berlin: Institut Bauen und Umwelt e.V., Product category rules on Guidance-Texts for Building-
2021. www.ibu-epd.com Related Products and Services. Part B: Requirements
on the EPD for Concrete components made of in-situ
No 528/2012 or ready-mixed concrete. Berlin: Institut Bauen und
Regulation (EU) No 528/2012 of the European Umwelt e.V. 21/03/2022
Parliament and of the Council of 22 May 2012
13 EPD Aggregate Industries – BWL2922/018 concrete, Plant Bow
Publisher
IBU - Institut Bauen und Umwelt e.V. Tel +49 (0)30 3087748 - 0
Hegelplatz 1 Fax +49 (0)30 3087748 - 29
10117 Berlin Mail info@ibu-epd.com
Germany Web www.ibu-epd.com
Programme holder
IBU - Institut Bauen und Umwelt e.V. Tel +49 (0)30 3087748 - 0
Hegelplatz 1 Fax +49 (0)30 3087748 - 29
10117 Berlin Mail info@ibu-epd.com
Germany Web www.ibu-epd.com
Author of the Life Cycle
Assessment
Climate Earth, Inc. Tel +1 (415) 391-2725
137 Park Place, Suite 204 Mail info@climateearth.com
Point Richmond, CA 94801 Web www.climateearth.com
United States
Owner of the Declaration
Aggregate Industries Tel +44 20 8380 7300
Bardon Hall Mail
LE67 1TL Coalville
United Kingdom london.concrete@aggregate.com
Web www.aggregate.com
14 EPD Aggregate Industries – BWL2922/018 concrete, Plant Bow
