ENVIRONMENTAL PRODUCT DECLARATION
as per ISO 14025 and EN 15804+A2
Owner of the Declaration dormakaba International Holding GmbH
Publisher Institut Bauen und Umwelt e.V. (IBU)
Programme holder Institut Bauen und Umwelt e.V. (IBU)
Declaration number EPD-DOR-20230450-CBA2-EN
Issue date 27.11.2023
Valid to 26.11.2028
Crane Manual Revolving Door - AL 1000/2000/3000
dormakaba
www.ibu-epd.com | https://epd-online.com
General Information
dormakaba Crane Manual Revolving Door - AL 1000/2000/3000
Programme holder Owner of the declaration
IBU – Institut Bauen und Umwelt e.V. dormakaba International Holding GmbH
Hegelplatz 1 DORMA Platz 1
10117 Berlin 58256 Ennepetal
Germany Germany
Declaration number Declared product / declared unit
EPD-DOR-20230450-CBA2-EN 1 piece of the product: Manual Revolving Door AL 1000/2000/3000, with a
diameter of 7 ft. (2130 mm) and a height of 7,5 ft. (2290 mm), consisting of
the following items:
• 4 door leaves
• Enclosure
• Canopy
• Product packaging
This declaration is based on the product category rules: Scope:
Automatic doors, automatic gates, and revolving door systems, This Environmental Product Declaration refers to a specific manual
01.08.2021 revolving door manufactured by dormakaba. The production site is located
(PCR checked and approved by the SVR) in Reamstown (USA).
The data represents the year 2022.
Issue date The owner of the declaration shall be liable for the underlying information
and evidence; the IBU shall not be liable with respect to manufacturer
27.11.2023
information, life cycle assessment data and evidences.
The EPD was created according to the specifications of EN 15804+A2. In
Valid to
the following, the standard will be simplified as EN 15804.
26.11.2028
Verification
The standard EN 15804 serves as the core PCR
Independent verification of the declaration and data according to ISO
14025:2011
internally X externally
Dipl.-Ing. Hans Peters
(Chairman of Institut Bauen und Umwelt e.V.)
Florian Pronold Matthias Klingler,
(Managing Director Institut Bauen und Umwelt e.V.) (Independent verifier)
1 Environmental Product Declaration - dormakaba - Crane Manual Revolving Door - AL 1000/2000/3000
Product
Product description/Product definition Base materials/Ancillary materials
The Crane AL 1000/2000/3000 Manual Revolving Doors allow The major material composition including the packaging of the
both greater traffic volume and quicker traffic flow compared to product is listed below:
automatic or manual swing doors. Crane manual revolving Name Value Unit
doors are customizable revolving doors. They enable a
Glass 43 %
continuous flow of traffic, especially in entrance areas, and at
Aluminium 35 %
the same time block the ingress of air from outside. A wide
selection of finishes is available to meet project needs. Steel 11 %
Zinc 7 %
For Crane Manual Revolving Doors AL 1000/2000/3000 the Plastics 4 %
standards which can be applied are the following:
The product includes partial articles which contain substances
• ANSI 156.27
listed in the Candidate List of REACH Regulation
1907/2006/EC (date: 14.06.2023) exceeding 0.1 percentage by
mass: no
Application
Revolving doors may be used to provide a comfortable entry
The Candidate List can be found on the ECHA website
and exit in many applications in the facade of or within a
address: https:echa.europa.eu/de/home.
building. Typical applications include:
• Hotels Reference service life
• Healthcare settings The reference service life of the Crane Manual Revolving Door
• Airports and transportation facilities AL 1000/2000/3000 amounts to 30 years, depending on the
• Commercial office buildings application and frequency of use. For repairs and renewals,
• Institutional and educational buildings suitable spare parts are available. The revolving door is tested
• Retail stores and certified to ANSI 156.27, meaning they are designed to
withstand a minimum of 1.000.000 cycles.
Technical Data
The Crane manual revolving doors AL 1000/2000/3000 have
following technical properties:
Name Value Unit
Height range 1000/2000 7-9 ft
Height range 3000 7+ ft
Diameter range maximum
12 ft
1000/2000/3000
clear or tinted
Enclosure glass 1000/2000 7/16"
laminated
clear or tinted
Enclosure glass 3000 9/16"
laminated
Door leaf glass 1/4" tempered
The product with respect to its characteristics is in accordance
with the relevant technical provisions (no CE-marking):
• ANSI 156.27
LCA: Calculation rules
Production - Module A1-A3
Declared Unit The product stage includes:
The declared unit is 1 piece of the product: Manual Revolving — A1, raw material extraction, processing and mechanical
Door AL 1000/2000/3000 including packaging treatments, processing of secondary material input (e.g.
Name Value Unit recycling processes),
— A2, transport to the manufacturer,
Declared unit 1 piece/product
— A3, manufacturing and assembly including provision of all
Mass of declared Product 591 kg
materials, products and energy, as well as waste processing up
to the end-of-waste state.
System boundary
The type of EPD is: cradle to gate with options, modules C1– Construction stage - Modules A4-A5
C4, and module D (A1–A3 + C + D and additional modules: The construction process stage includes:
A4+ A5) — A4, transport to the building site;
— A5, installation into the building;
including provision of all materials, products and energy, as well
as waste processing up to the end-of-waste state or disposal of
final residues during the construction process stage.
2 Environmental Product Declaration - dormakaba - Crane Manual Revolving Door - AL 1000/2000/3000
End-of-life stage– Modules C1-C4 and D Geographic Representativeness
The end-of-life stage includes: Land or region, in which the declared product system is
— C1, de-construction, demolition: manufactured, used or handled at the end of the product´s
— C2, transport to waste processing; lifespan: Global
— C3, waste processing for reuse, recovery and/or recycling;
— C4, disposal;
Comparability
including provision and all transport, provision of all materials,
Basically, a comparison or an evaluation of EPD data is only
products and related energy and water use.
possible if all the data sets to be compared were created
according to EN 15804 and the building context, respectively
Module D (Benefits and loads beyond the system boundary)
the product-specific characteristics of performance, are taken
includes:
into account. Background database: GaBi, SP40.
— D, recycling potentials, expressed as net impacts and
benefits.
LCA: Scenarios and additional technical information
Reference service life
Characteristic product properties of biogenic carbon
Name Value Unit
Information on describing the biogenic carbon content at
Life Span according to the manufacturer 30 a
factory gate
Name ValueUnit End of life (C1-C4)
kg C1: The product expansion depends on the building. The
Biogenic carbon content in product -
C product share is so low that no environmental burden is
Biogenic carbon content in accompanying kg assumed.
-
packaging C C2: Transport to waste management is 50 km.
Note: 1 kg of biogenic carbon is equivalent to 44/12 kg of CO . Name Value Unit
2
Collected separately waste type waste type 582 kg
Recycling 316 kg
Energy recovery 14.2 kg
Transport to the building site (A4) Landfilling 252 kg
Name Value Unit The product is disassembled in a recycling process. Material
Litres of fuel 0.00276 l/100km recycling is then assumed for the metals and electronics. The
Transport distance 50 km plastic components are assumed to be incinerated with energy
recovery. Minor proportions of residues arising from the
Capacity utilisation (including empty runs) 55 %
recycling process are landfilled. Region for the End of Life is:
The product is transported via truck. The main distribution Global.
region is North America. In order to allow scaling to a specific
point of installation 100 km are declared.
Reuse, recovery and/or recycling potentials (D), relevant
scenario information
Installation into the building (A5)
Name Value Unit
Name Value Unit
Recycling 100 %
Waste packaging (paper and plastic) 9 kg
The collection rate is 100 %.
3 Environmental Product Declaration - dormakaba - Crane Manual Revolving Door - AL 1000/2000/3000
LCA: Results
DESCRIPTION OF THE SYSTEM BOUNDARY (X = INCLUDED IN LCA; MND = MODULE OR INDICATOR NOT DECLARED; MNR
= MODULE NOT RELEVANT)
Benefits and
Construction loads beyond
Product stage Use stage End of life stage
process stage the system
boundaries
la ire ta m w a Ry lp p u s tro p s n a rT g n iru tc a fu n a M e h t m o rf tro p s n a rTe tis e h t o t e ta g y lb m e s s A e s U e c n a n e tn ia M ria p e R tn e m e c a lp e R tn e m h s ib ru fe R y g re n e la n o ita re p Oe s u re ta w la n o ita re p Oe s u n o itc u rts n o c -e Dn o itilo m e d tro p s n a rT g n is s e c o rp e ts a W la s o p s iD -e s u e R-y re v o c e R-g n ilc y c e Rla itn e to p
A1 A2 A3 A4 A5 B1 B2 B3 B4 B5 B6 B7 C1 C2 C3 C4 D
X X X X X MND MND MNR MNR MNR MND MND X X X X X
RESULTS OF THE LCA - ENVIRONMENTAL IMPACT according to EN 15804+A2: 1 piece Crane AL 1000/2000/3000
Parameter Unit A1-A3 A4 A5 C1 C2 C3 C4 D
GWP-total kg CO 2 eq 3.27E+03 5.17E+00 2.29E+01 0 2.55E+00 4.06E+01 3.85E+00 -1.49E+03
GWP-fossil kg CO 2 eq 3.26E+03 4.94E+00 2.29E+01 0 2.43E+00 4.06E+01 3.83E+00 -1.49E+03
GWP-biogenic kg CO 2 eq 3.07E+00 2.28E-01 5.33E-04 0 1.12E-01 9.45E-04 1.3E-02 -4.57E+00
GWP-luluc kg CO 2 eq 1.28E+00 1.18E-04 1E-03 0 5.79E-05 2E-03 1.1E-02 -2.71E-01
ODP kg CFC11 eq 2.32E-11 5.22E-16 1.15E-14 0 2.57E-16 2.05E-14 1.42E-14 -1.02E-08
AP mol H+ eq 1.41E+01 5E-03 4E-03 0 2E-03 7E-03 2.7E-02 -5.6E+00
EP-freshwater kg P eq 2.48E-03 1.06E-06 1.84E-06 0 5.21E-07 3.26E-06 6.57E-06 -1E-03
EP-marine kg N eq 2.31E+00 2E-03 9.18E-04 0 7.75E-04 2E-03 7E-03 -7.46E-01
EP-terrestrial mol N eq 2.55E+01 1.7E-02 1.9E-02 0 9E-03 3.3E-02 7.8E-02 -8.05E+00
kg NMVOC
POCP 6.32E+00 4E-03 3E-03 0 2E-03 5E-03 2.1E-02 -2.43E+00
eq
ADPE kg Sb eq 1.43E-01 1.48E-07 1.58E-07 0 7.3E-08 2.81E-07 3.44E-07 -5.5E-02
ADPF MJ 4.64E+04 7.01E+01 1.06E+01 0 3.45E+01 1.88E+01 5.02E+01 -2.06E+04
m3 world eq
WDP 5.11E+02 1E-02 2.34E+00 0 5E-03 4.15E+00 4.01E-01 -8.93E+01
deprived
GWP = Global warming potential; ODP = Depletion potential of the stratospheric ozone layer; AP = Acidification potential of land and water; EP =
Eutrophication potential; POCP = Formation potential of tropospheric ozone photochemical oxidants; ADPE = Abiotic depletion potential for non-fossil
resources; ADPF = Abiotic depletion potential for fossil resources; WDP = Water (user) deprivation potential)
RESULTS OF THE LCA - INDICATORS TO DESCRIBE RESOURCE USE according to EN 15804+A2: 1 piece Crane AL
1000/2000/3000
Parameter Unit A1-A3 A4 A5 C1 C2 C3 C4 D
PERE MJ 1.37E+04 2.21E-01 2.76E+00 0 1.09E-01 4.89E+00 6.58E+00 -8.99E+03
PERM MJ 0 0 0 0 0 0 0 0
PERT MJ 1.37E+04 2.21E-01 2.76E+00 0 1.09E-01 4.89E+00 6.58E+00 -8.99E+03
PENRE MJ 4.56E+04 7.01E+01 3.98E+02 0 3.45E+01 5.28E+02 5.02E+01 -2.06E+04
PENRM MJ 8.96E+02 0 -3.87E+02 0 0 -5.09E+02 0 0
PENRT MJ 4.65E+04 7.01E+01 1.06E+01 0 3.45E+01 1.88E+01 5.02E+01 -2.06E+04
SM kg 2.16E+00 0 0 0 0 0 0 0
RSF MJ 0 0 0 0 0 0 0 0
NRSF MJ 0 0 0 0 0 0 0 0
FW m3 3.27E+01 3.96E-04 5.6E-02 0 1.95E-04 9.9E-02 1.3E-02 -1.61E+01
PERE = Use of renewable primary energy excluding renewable primary energy resources used as raw materials; PERM = Use of renewable primary
energy resources used as raw materials; PERT = Total use of renewable primary energy resources; PENRE = Use of non-renewable primary energy
excluding non-renewable primary energy resources used as raw materials; PENRM = Use of non-renewable primary energy resources used as raw
materials; PENRT = Total use of non-renewable primary energy resources; SM = Use of secondary material; RSF = Use of renewable secondary fuels;
NRSF = Use of non-renewable secondary fuels; FW = Use of net fresh water
RESULTS OF THE LCA – WASTE CATEGORIES AND OUTPUT FLOWS according to EN 15804+A2:
1 piece Crane AL 1000/2000/3000
Parameter Unit A1-A3 A4 A5 C1 C2 C3 C4 D
HWD kg 3.08E-05 6.8E-09 4.04E-08 0 3.35E-09 7.17E-08 7.65E-07 -1.85E-04
NHWD kg 5.85E+02 7E-03 2.38E+00 0 4E-03 4.21E+00 2.52E+02 -3.25E+02
RWD kg 2.93E+00 7.53E-05 3.94E-04 0 3.71E-05 6.98E-04 5.72E-04 -2.15E+00
CRU kg 0 0 0 0 0 0 0 0
MFR kg 0 0 0 0 0 3.14E+02 0 0
MER kg 0 0 0 0 0 0 0 0
EEE MJ 0 0 4.24E+01 0 0 7.51E+01 0 0
EET MJ 0 0 9.73E+01 0 0 1.72E+02 0 0
4 Environmental Product Declaration - dormakaba - Crane Manual Revolving Door - AL 1000/2000/3000
HWD = Hazardous waste disposed; NHWD = Non-hazardous waste disposed; RWD = Radioactive waste disposed; CRU = Components for re-use;
MFR = Materials for recycling; MER = Materials for energy recovery; EEE = Exported electrical energy; EET = Exported thermal energy
RESULTS OF THE LCA – additional impact categories according to EN 15804+A2-optional:
1 piece Crane AL 1000/2000/3000
Parameter Unit A1-A3 A4 A5 C1 C2 C3 C4 D
Disease
PM 1.29E-04 2.6E-08 5.2E-08 0 1.28E-08 9.22E-08 3.4E-07 -8.84E-05
incidence
IR kBq U235 eq 4.3E+02 1.1E-02 3.5E-02 0 5E-03 6.3E-02 5.9E-02 -4.26E+02
ETP-fw CTUe 2.24E+04 4.97E+01 3.98E+00 0 2.45E+01 7.06E+00 2.87E+01 -7.57E+03
HTP-c CTUh 1.95E-06 9.34E-10 3.45E-10 0 4.6E-10 6.11E-10 4.25E-09 2.06E-07
HTP-nc CTUh 4.66E-05 4E-08 3.49E-08 0 1.97E-08 6.19E-08 4.68E-07 4.87E-05
SQP SQP 3.84E+03 1.8E-01 3.18E+00 0 8.9E-02 5.63E+00 1.05E+01 -5.95E+02
PM = Potential incidence of disease due to PM emissions; IR = Potential Human exposure efficiency relative to U235; ETP-fw = Potential comparative
Toxic Unit for ecosystems; HTP-c = Potential comparative Toxic Unit for humans (cancerogenic); HTP-nc = Potential comparative Toxic Unit for humans
(not cancerogenic); SQP = Potential soil quality index
Disclaimer 1 – for the indicator “Potential Human exposure efficiency relative to U235”. This impact category deals mainly with the
eventual impact of low-dose ionizing radiation on human health of the nuclear fuel cycle. It does not consider effects due to possible
nuclear accidents, occupational exposure or radioactive waste disposal in underground facilities. Potential ionizing radiation from the
soil, radon and from some construction materials is also not measured by this indicator.
Disclaimer 2 – for the indicators “abiotic depletion potential for non-fossil resources”, “abiotic depletion potential for fossil resources”,
“water (user) deprivation potential, deprivation-weighted water consumption”, “potential comparative toxic unit for ecosystems”,
“potential comparative toxic unit for humans – cancerogenic”, “Potential comparative toxic unit for humans - not cancerogenic”,
“potential soil quality index”. The results of this environmental impact indicator shall be used with care as the uncertainties on these
results are high as there is limited experience with the indicator.
This EPD was created using a software tool.
References
ANSI 156.27 GaBi ts documentation
ANSI/BHMA A156.27-2019, Power and Manual Operated GaBi life cycle inventory data documentation
Revolving Pedestrian Doors (https://www.gabisoftware.com/support/gabi/gabidatabase-
2020-lcidocumentation/).
EN 15804
EN 15804+A2:2019+AC:2021, LCA-tool dormakaba
Sustainability of construction works — Environmental Product Tool No.: IBU-DOR-202107-LT1-EN .
Declarations — Core rules for the product category of Developed by Sphera Solutions GmbH
construction products
PCR Part A
ISO 14025 PCR – Part A: Calculation Rules for the Life Cycle Assessment
DIN EN ISO 14025:201110, Environmental labels and and Requirements on the Project Re-port according to EN
declarations — Type III environmental declarations — 15804+A2:2019, Version 1.0, 2020, Institut Bauen und Umwelt
Principles and procedures e.V., www.ibu-epd.com.
REACH PCR Part B
Regulation (EC) No 1907/2006 of the European Parliament and PCR – Part B: Requirements on the EPD for Automatic doors,
of the Council on the Registration, Evaluation, Authorisation automatic gates, and revolving door systems, version 5, 2023,
and Restriction of Chemicals (REACH) Institut Bauen und Umwelt e.V.,
www.ibu-epd.com.
Further References
IBU 2021
General Instructions for the EPD programme of Institut Bauen
und Umwelt e.V. Version 2.0, Berlin: Institut Bauen und Umwelt
e.V., 2021. www.ibu-epd.com
GaBi
Sphera Solutions GmbH
Gabi Software System and Database for Life Cycle Engineering
19922020
Version 10.0.0.71
University of Stuttgart
Leinfelden-Echterdingen
5 Environmental Product Declaration - dormakaba - Crane Manual Revolving Door - AL 1000/2000/3000
Publisher
Institut Bauen und Umwelt e.V. +49 (0)30 3087748- 0
Hegelplatz 1 info@ibu-epd.com
10117 Berlin www.ibu-epd.com
Germany
Programme holder
Institut Bauen und Umwelt e.V. +49 (0)30 3087748- 0
Hegelplatz 1 info@ibu-epd.com
10117 Berlin www.ibu-epd.com
Germany
Author of the Life Cycle Assessment
dormakaba International Holding GmbH +49 2333 793-0
DORMA Platz 1 info.de@dormakaba.com
58256 Ennepetal www.dormakaba.com
Germany
Owner of the Declaration
dormakaba International Holding GmbH +49 2333 793-0
DORMA Platz 1 info.de@dormakaba.com
58256 Ennepetal www.dormakaba.com
Germany
6 Environmental Product Declaration - dormakaba - Crane Manual Revolving Door - AL 1000/2000/3000
