DAPHabitat System Environmental Product Declaration
www.daphabitat.pt
[according to ISO 14025, EN 15804:2012+A2:2019 and EN 15942]
Declaration number: DAP 001:2023
COLD-FORMED WELDED STRUCTURAL HOLLOW SECTIONS OF
NON-ALLOY AND FINE GRAINS STEELS
Issue date: 02/05/2023 Valid until: 01/05/2028
FERPINTA - INDÚSTRIAS DE TUBOS DE AÇO DE FERNANDO PINHO TEIXEIRA, S.A.
VERSION 1.2. EDITION JUNE 2022
Índice
1. GENERAL INFORMATION ............................................................................................................................... 1
1.1. THE DAPHABITAT SYSTEM ....................................................................................................................................... 1
1.2. EPD OWNER ......................................................................................................................................................... 1
1.3. INFORMATION CONCERNING THE EPD ........................................................................................................................ 2
1.4. DEMONSTRATION OF THE VERIFICATION ...................................................................................................................... 2
1.5. EPD REGISTRATION ................................................................................................................................................ 2
1.6. RELEVANTE C-PCR (COMPLEMENTARY PRODUCT CATEGORY RULES) ................................................................................ 3
1.7. INFORMATION CONCERNING THE PRODUCT/PRODUCT CLASS .......................................................................................... 3
1.8. CALCULATION RULES OF THE LCA .............................................................................................................................. 4
1.9. USE OF AVERAGE ENVIRONMENTAL PERFORMANCE ....................................................................................................... 5
1.10. TECHNICAL INFORMATION FOR REFERENCE SERVICE LIFE (RSL) ..................................................................................... 5
1.11. FLOW DIAGRAM OF INPUT AND OUTPUT OF THE PROCESSES .......................................................................................... 6
2. CORE ENVIRONMENTAL IMPACT INDICATORS ............................................................................................... 7
2.1. DESCRIPTION OF THE SYSTEM BOUNDARIES ................................................................................................................. 7
2.1.1. JUSTIFICATION FOR THE EXEMPTION TO DECLARE MODULE C1, C2, C3, C4 AND D .......................................................... 8
2.2. CORE ENVIRONMENTAL IMPACT INDICATORS ............................................................................................................... 8
2.3. ADDITIONAL ENVIRONMENTAL IMPACT INDICATORS .................................................................................................... 10
2.4. INDICATORS DESCRIBING RESOURCE USE ................................................................................................................... 11
2.5. OTHER ENVIRONMENTAL INFORMATION DESCRIBING DIFERENTE WASTE CATEGORIES ........................................................ 12
2.6. ENVIRONMENTAL INFORMATION DESCRIBING OUTPUT FLOWS ...................................................................................... 12
2.7. INFORMATION DESCRIBING THE BIOGENIC CARBON CONTENT AT THE FACTORY GATE ......................................................... 13
3. SCENARIOS AND ADDITIONAL TECHNICAL INFORMATION ............................................................................13
3.1. C2 TRANSPORT – END OF LIFE OF THE PRODUCT ......................................................................................................... 13
3.2. C3 WASTE PROCESSING FOR REUSE, RECOVERY AND/OR RECYCLING – END OF LIFE OF THE PRODUCT ................................... 13
3.3. C4 DISPOSAL – END OF LIFE OF THE PRODUCT ............................................................................................................ 13
3.4. SCENARIO AND TECHNICAL INFORMATION FOR MODULE D ........................................................................................... 14
3.5. ADDITIONAL INFORMATION ON RELEASE OF DANGEROUS SUBSTANCES TO INDOOR AIR, SOIL, AND WATER DURING THE USE STAGE
................................................................................................................................................................................ 14
REFERENCES .........................................................................................................................................................15
DAPHabitat System iii
1. GENERAL INFORMATION
1.1. The DAPHabitat System
Programme operator:
Sustainable Construction Platform
www.centrohabitat.net
centrohabitat@centrohabitat.net
Address: Departamento Engenharia Civil
Universidade de Aveiro
3810-193 Aveiro
Email address: deptecnico@centrohabitat.net
Telephone number: (+351) 234 401 576
Website: www.daphabitat.pt
Logo:
1.2. EPD Owner
Name of the owner: FERPINTA – Indústrias de Tubos de Aço de Fernando Pinho Teixeira, S.A.
Production site: Rua 13 de Julho, nº295
3720-011 Carregosa, Oliveira de Azeméis
Address (head office): Rua 13 de Julho, nº295
3720-011 Carregosa, Oliveira de Azeméis
Telephone: 256 411 420
E-mail: infor@ferpinta.pt
ana.amorim.fer@ferpinta.pt
Website: www.ferpinta.pt
Logo:
Information concerning the NP EN ISO 9001:2015 – Quality Management Systems
applicable management systems: NP EN ISO 14001:2015 – Environmental Management System
NP EN ISO 50001:2019 – Energy Management Systems
Specific aspects regarding the Main CAE: 24200 – Manufacture of tubes, pipes, hollow profiles and related fittings, of steel
productin:
Organization’s environmental FERPINTA aims to build a better future by producing pipes, profiles, shapes, and bands of
policy: steel that we want to get further and further. Aware of its mission, FERPINTA seeks to adopt
methods and technologies that prevent pollution protect the environment, using natural
resources in an effective way, and ensuring that FERPINTA products are developed
considering the life cycle perspective. The full Management Policy can be consulted at:
www.grupoferpinta.com/imagem/PolíticaGestão_FPT.pdf.
DAPHabitat System 1
1.3. Information concerning the EPD
Authors: Ana Cláudia Dias
Contact of the authors: Endereço: Universidade de Aveiro, Campus Universitário de Santiago, 3810-193 Aveiro, Portugal
Telefone: 234 370 200
E-mail: acdias@ua.pt
Issue date: 02/05/2023
Registration date: 22/05/2023
Registration number: DAP 001:2023
Valid until: 01/05/2028
Representativity of the
EPD(location, manufacturer, EPD of one (1) product category, produced in one (1) industrial plant from one (1) producer
group of manufacturers):
Where to consult explanatory
www.ferpinta.pt
material:
Type of EPD: Cradle-to-gate EPD (A1-A3) with modules C and D
1.4. Demonstration of the verification
External independent verification, accordingly with the standard ISO 14025:2009 and EN 15804:2012+A2:2019
Certification Body Verifier
(CERTIF – Associação para a Certificação ) (Marisa Almeida)
1.5. EPD Registration
Programme Operator
(Plataforma para a Construção Sustentável)
2 DAPHabitat System
1.6. Relevante c-PCR (complementary product category rules)
Not applicable.
1.7. Information concerning the product/product class
Identification of the product: Cold-formed welded structural hollow sections of non-alloy and fine steel grains steels
Ilustration of the product:
Brief description of the product: FERPINTA’s range of structural hollow sections consists of round, square, and rectangular
products, longitudinally welded, cold-formed, and without subsequent heat treatment.
Structural hollow sections are produced according to the EN 10219-1 standard, with a
diameter range of 16 to 323.9 mm, and with a wall thickness of 1.5 to 12.5 mm. The tube can
be supplied in black (rough rolled) or pickled. The entire range of cold-formed welded
structural hollow sections produced at FERPINTA is included in the EPD.
Main technical characteristics of The technical properties of the cold-formed welded structural hollow sections comply with the
the product: requirements of the EN 10219-1:2006 and EN 10219-2:2006 standards, as indicated in Table 1.
The mechanical properties are presented in Table 2.
Table 1: General properties
Properties Standard Section
Tolerances on dimension and shape EN 10219-2 6
Elongation EN 10219-1 6.7.1, Tables A.3, B.4 and B.5
Tensile strength and yield strength EN 10219-1 6.7.1, Tables A.3, B.4 and B.5
Impact strength EN 10219-1 6.7.2, Tables A.3, B.4 and B.5
Weldability EN 10219-1 6.6, Tables A.1, B.1, B.2 and 6.8.1
Durability EN 10219-1 6.8.2
Table 2: Mechanical properties, according to the EN 10219-1:2006 standard
Mechanical properties
Minimum
Minimum Minimum impact energy, KV
Steel
yield Tensile strength, Rm
elongation, A (J)
strength, (MPa)
grade (%))
ReH (MPa)
Thickness (mm) At test temperature of
≤ 16mm < 3 ≥ 3 ≤ 40 ≤ 40 -50 ◦C -20 ◦C 0 ◦C 20 ◦C
S235JRH 235 360-510 360-510 24 - - - 27
S275J0H 275 430-580 410-560 20 - - 27 -
S275J2H 275 430-580 410-560 20 - 27 - -
S355J0H 355 510-680 470-630 20 - - 27 -
S355J2H 355 510-680 470-630 20 - 27 - -
S355K2H 355 510-680 470-630 20 - 40 - -
S420MH 420 - 500-660 19 - 40 - -
S420MLH 420 - 500-660 19 27 - - -
S460MH 460 - 530-720 17 - 40 - -
S460MLH 460 - 530-720 17 27 - - -
S460NH 460 - 540-720 17 - 40 - -
S460NLH 460 - 540-720 17 27 - - -
Note: specific information in the technical sheet of the product and/or on the label.
DAPHabitat System 3
Description of the product’s For use in metallic structures or mixed structures - metal and concrete.
application/use:
Placing on the market / Rules of • EN 10219;
application in the market / • Certificate of conformity of the factory production control, according to Regulation
Technical rules of the product: 305/2011/EU.
Quality control: According to EN 10219-1, Section 7.3, Table 2 – Inspection programme for hollow sections of
non-alloy steels (specific inspection).
Special delivery conditions: Not applicable.
Components and substances to Not applicable.
declare:
Other information about the The cold-formed welded structural hollow sections are one of the most versatile and efficient
product: solutions when it comes to metallic and composite construction, or even mechanical
applications. With its use, it becomes possible to obtain lightweight, dynamic, and resistant
structures, with excellent performance in compression. They allow use in large spans and have
a high strength-to-weight ratio. The structural hollow sections produced by FERPINTA can be
supplied in special lengths, and may also comply with specific requirements with regard to
suitability for hot-dip galvanization, weldability at the corners according to Eurocode 3 (EC3,)
and specific carbon equivalent value (CEV)..
History of the LCA studies: -
1.8. Calculation rules of the LCA
Functional unit: Not applicable
Declared unit: 1 tonne (t) of cold-formed welded structural hollow sections, with a density of 7,850 kg/m3,
ready for delivery.
System boundaries: The assessed system includes modules A1-A3 (product stage), C (end of life stage), and D
(benefits and loads beyond the system boundary). In module C, the impacts of submodule C1
(deconstructions and demolition) were excluded due to the lack of information. A more
detailed description of the system boundary is presented in Section 2.1.
Criteria for the exclusion: The LCA considered all the production processes of the materials and energy consumed in
the system, as well as the management processes of the wastes generated, for which
inventory data were available. It should be noted that the flows of materials excluded in the
structural hollow sections production process are equal to 0.02% of the total mass of inputs
to that process and, therefore, are covered by the cut-off criteria defined in the ‘PCR – Basic
Model’ document. More specifically, their mass contributes less than 1% to the total mass of
the inputs and less than 5% to the total mass of inputs to each information module.
The consumption of energy and water in the administrative areas, as well as the production
of wastewater and wastes from these areas, were excluded. The environmental burdens
from the construction and maintenance of infrastructures and equipment (capital goods)
were also excluded, except those associated with the maintenance of machinery and
equipment used in the production of structural hollow sections.
Assumption and limitations: The results of the environmental impacts and remaining indicators shown in this EDP refer to
the year 2020 and constitute average values for the entire range of cold-formed welded
structural hollow sections produced by FERPINTA. The calculation software does not allow
quantifying the indicators describing waste categories for all declared modules, from a life
cycle perspective.
Quality and other characteristics For the production process of cold-formed welded structural hollow sections, real and
about the information used in the specific data from the production plant have been used. The only exception is emissions to
LCA: air resulting from the burning of diesel consumed in internal transport operations, which
have been calculated based on emission factors due to the lack of measured values.
For the remaining processes, such as steel production and electricity production in the grid,
generic data obtained from the Ecoinvent database have been used, which meet the quality
criteria defined for generic data (time-related, geographical and technological
4 DAPHabitat System
representativeness, plausibility, completeness, consistency, etc.). Whenever possible, the
original processes from Ecoinvent were adapted to better represent reality, for example by
changing the mix of energy sources of electricity consumed considering the country where
processes take place.
According to the criteria defined in Table E.1 of Annex E of the EN 15804 standard, defined
by “UN Environment Global Guidance on LCA database development”, the quality of all
relevant data is very good. The quality of the data used in module D is also very good, except
for the geographical representativeness of some processes, which is considered good.
Allocation rules: In addition to cold-formed welded structural hollow sections, FERPINTA also produces other
types of tubes, which constitutes a multifunctionality situation. To determine the inputs and
outputs associated only with the production of cold-formed welded structural hollow
sections, the unit process subdivision procedure was first adopted. Therefore, only
operations associated with the production of the product under assessment were considered
and the operations associated with the remaining products were excluded. Then, for the
included operations, an allocation procedure based on the mass of the different products
produced was applied.
In the production process of cold-formed welded structural hollow sections, there is also
multifunctionality associated with recycling. On the one hand, part of the steel consumed is
produced from scrap; the environmental impacts from the production of this steel refer to
the operations that take place after the collection and sorting of the scrap. On the other
hand, some waste will be subsequently recovered, for which further processing was
considered until they reach the end of waste state.
The structural hollow sections at the end of life are recycled. Also in this case, their further
processing until they reach the end of waste state was considered.
Software used for the assessment: SimaPro version 9.2.0.2.
Background database used for the Ecoinvent version 3.7.1 database published in December 2020; “cut-off” approach.
LCA:
Comparability of EPD for The EPD of construction products and services cannot be comparable in case they are not
construction products: produced according to EN 15804 and EN 15948 and according to the comparability
conditions determined by ISO 14025.
1.9. Use of average environmental performance
This EPD presents the average environmental performance of the entire range of cold-formed welded structural
hollow sections produced by FERPINTA in 2020. The variability of the environmental performance between specific
products is not relevant.
1.10. Technical information for Reference Service Life (RSL)
Not applicable.
DAPHabitat System 5
1.11. Flow diagram of input and output of the processes
A1 -extraction and processing of raw materials
A2 - transport
A3 -manufacturing
Reception of raw material
Longitudinal cut
s
e
c n
re
w Materials for
a o
n e tn
ia
Tube production g n ilot recycling
M o
C
Storage
Despatch
Cold-formed welded structural
hollow sections
C -end of life
C2: transport Materials for
C3: waste processing recycling
C4: waste disposal
D -benefits and loads beyond the system boundary
Recycling of structural hollow sections at the end of life
Recycling of steel scrap from the manufacturing process
System boundaries
Figure 1: Life cycle stages and unit processes of the product
6 DAPHabitat System
2. CORE ENVIRONMENTAL IMPACT INDICATORS
2.1. Description of the system boundaries
(✓= included; ND = module not declared)
CONSTRUCTIO BENEFITS AND LOADS
PRODUCT STAGE N PROCESS USE STAGE END OF LIFE STAGE BEYOND THE SYSTEM
STAGE BOUNDARY
y lp p u s la ire ta m w a R tro p s n a rT g n iru tc a fu n a M tro p s n a rT
s s
e c o rp n o ita lla ts n i n o itc u rts n
o C
e s U e c n a n e tn ia M ria p e R tn e m e c a lp e R tn e m h s ib ru fe R e s u y g re n e la n o ita re p O e s u re ta w la n o ita re p O n o itilo m e d ,s n o itc u rts n eo Dc - tro p s n a rT g n is s e c o rp e ts a W la s o p s iD
la
itn
e to p g n ilc y c e r ,y re v o c e r ,e
es Ru -
A1 A2 A3 A4 A5 B1 B2 B3 B4 B5 B6 B7 C1 C2 C3 C4 D
✓ ✓ ✓ ND ND ND ND ND ND ND ND ND ND ✓ ✓ ✓ ✓
Module A1-A3 (product stage) considers the manufacturing of structural hollow sections, as well as the extraction, processing, and transport of
raw material (hot rolled steel coils), ancillary materials, packaging materials, and energy vectors, and also waste processing until the end of
waste state is reached or until the end of life.
The manufacturing process of structural hollow sections starts with raw material reception (steel coils) where the properties of the material are
confirmed. The next operation is longitudinal cutting where steel coils are cut in strips with width compatible with the diameters/dimensions of
the hollow sections to be produced. After this operation, the material enters in the tube production/conformation line.
The strip resulting from the longitudinal cutting operation are unrolled and sent to conformation (when a slit is unrolled, the slits are connected
by butt joint welding). In the hollow section conformation is used a set of rollers that gives the strip the configuration near of a circle, lightly
open on the edge. The next operation is the longitudinal electric resistance welding, where the outer excesses of the weld are eliminated by
rectification. The tube, continuously moving, is cooled and calibrated to achieve the intended cross-section – circular, rectangular or square,
according to the normative requirements. Before cutting in the intended length, a protective oil may be applied for protection against
corrosion. The next operations are storage and expedition.
• In module C (end of life stage), the impacts from submodule C1 (deconstruction and demolition) were excluded because, although
mechanized deconstruction and demolition of structures built with the structural hollow sections may occur, there is no information
available allowing the quantification of the respective impacts. The following submodules were considered in module C:
• C2 – includes the transport of the structural hollow sections from the place of deconstruction or demolition until the end of life
(recycling);
• C3 – includes the activities taking place before recycling, in particular, sorting and pressing of the hollow sections;
• C4 – corresponds to waste final disposal; the environmental impacts are null as the hollow sections are recycled.
Module D considers the environmental benefits and loads associated with recycling the structural hollow sections at the end of life and of the
steel scrap generated in the hollow sections manufacturing process, assuming that steel recycling will avoid the production of steel from
primary material.
DAPHabitat System 7
2.1.1. Justification for the exemption to declare module C1, C2, C3, C4 and D
Not applicable.
2.2. Core environmental impact indicators
Depletion
Global Global Global warming
Global warming potential of
warming warming potential, land Acidification
potential, the
potential, potential, use and land use potential;
biogenic; stratospheric
total; fossil; change;
ozone layer;
AP
GWP-biogenic
GWP-total GWP-fossil GWP-luluc
ODP
Unit kg CO2 eq. kg CO2 eq. kg CO2 eq. kg CO2 eq. kg CFC 11 eq. mol H+ eq.
Modules A1-A3 2,50E+03 2,47E+03 2,87E+01 1,23E+00 1,22E-04 1,08E+01
Module C2 4,15E+01 4,14E+01 3,31E-02 3,14E-04 9,61E-06 1,43E-01
Module C3 1,29E+01 1,27E+01 1,32E-01 1,72E-02 2,15E-06 1,19E-01
Module C4 0,00E+00 0,00E+00 0,00E+00 0,00E+00 0,00E+00 0,00E+00
Module D -1,43E+03 -1,41E+03 -1,87E+01 4,39E-01 -5,06E-05 -5,23E+00
LEGEND:
Product Stage
End-of-life stage
Benefits and loads beyond the system boundary
NOTE:
Values expressed by declared unit (1 t of cold-formed welded structural hollow sections).
8 DAPHabitat System
Abiotic Abiotic
Eutrophication Eutrophication Eutrophication Formation
depletion depletion
potential potential potential potential of potential for potential for Water (user)
deprivation
aquatic aquatic terrestrial; tropospheric non-fossil fossil
potential;
freshwater; marine; ozone; resources resources
EP- potential
WDP
EP-freshwater EP-marine terrestrial POCP ADP-
minerals&metals ADP-fossil
m3 World eq.
Units kg P eq. kg N eq. mol N eq. Kg COVNM eq. kg Sb eq. MJ, P.C.I
deprived
Modules A1-A3 1,13E-01 2,26E+00 2,46E+01 1,13E+01 2,65E-02 2,59E+04 7,46E+02
Module C2 2,26E-05 4,60E-02 5,06E-01 1,38E-01 1,76E-06 5,87E+02 -1,24E-01
Module C3 2,09E-04 4,55E-02 5,00E-01 1,36E-01 4,92E-07 1,98E+02 1,10E+00
Module C4 0,00E+00 0,00E+00 0,00E+00 0,00E+00 0,00E+00 0,00E+00 0,00E+00
Module D -6,99E-02 -1,10E+00 -1,21E+01 -6,70E+00 -2,40E-02 -1,24E+04 -6,48E+01
LEGEND:
Product Stage
End-of-life stage
Benefits and loads beyond the system boundary
NOTES:
P.C.I. – Net calorific value
Values expressed by declared unit (1 t of cold-formed welded structural hollow sections).
The results of the indicators “Abiotic depletion potential for non-fossil resources”, “Abiotic depletion potential for fossil resources potential”, and “Water
(user) deprivation potential” shall be used with care as the uncertainties on these results are high or as there is limited experienced with the indicator.
DAPHabitat System 9
2.3. Additional environmental impact indicators
Potential Potential
Potential Potential Potential
incidence of human Comparative
Comparative Comparative Toxic Potential soil
disease due exposure Toxic Unit for
Toxic Unit for Unit for humans, quality index
to PM efficiency humans, not
ecosystems cancer effects
emissions relative to U235 cancer effects
SQP
IRP ETP-fw HTP-c
PM HTP-nc
Disease
Units kBq U 235 eq. CTUe CTUh CTUh -
incidence
Modules A1-A3 ND ND ND ND ND ND
Module C2 ND ND ND ND ND ND
Module C3 ND ND ND ND ND ND
Module C4 ND ND ND ND ND ND
Module D ND ND ND ND ND ND
LEGEND:
Product Stage
End-of-life stage
Benefits and loads beyond the system boundary
NOTES:
Values expressed by declared unit (1 t of cold-formed welded structural hollow sections).
The impact indicator “POTENTIAL HUMAN EXPOSURE EFFICIENCY RELATIVE TO U235” deals mainly with the eventual impact of low dose ionising
radiation on human health resulting of the nuclear fuel cycle. It does not consider effects due to possible nuclear accidents, occupational exposure nor
due to radioactive waste disposal in underground facilities. Potential ionising radiation from the soil, radon and some building materials is also not
measured by this indicator.
The results of the indicators “POTENTIAL COMPARATIVE TOXIC UNIT FOR ECOSYSTEMS”, “POTENTIAL COMPARATIVE TOXIC UNIT FOR HUMANS,
CANCER EFFECTS”, “POTENTIAL COMPARATIVE TOXIC UNIT FOR HUMANS, NOT CANCER EFFECTS” and “POTENTIAL SOIL QUALITY INDEX” shall be used
with care as the uncertainties on these results are high or as there is limited experience with the indicator.
.
10 DAPHabitat System
2.4. Indicators describing resource use
Secondary materials and fuels, and use of
Primary energy
water
Net use of
EPR RR TRR EPNR RNR TRNR MS CSR CSNR fresh
water
Unit MJ, P.C.I. MJ, P.C.I. MJ, P.C.I. MJ, P.C.I. MJ, P.C.I. MJ, P.C.I. kg MJ, P.C.I. MJ, P.C.I. m3
Modules A1-A3 2,24E+03 6,22E+01 2,31E+03 2,59E+04 5,09E+01 2,59E+04 2,19E+01 0,00E+00 0,00E+00 1,34E+01
Module C2 8,63E-01 0,00E+00 8,63E-01 5,87E+02 0,00E+00 5,87E+02 0,00E+00 0,00E+00 0,00E+00 8,81E-04
Module C3 1,35E+01 0,00E+00 1,35E+01 1,98E+02 0,00E+00 1,98E+02 0,00E+00 0,00E+00 0,00E+00 2,90E-02
Module C4 0,00E+00 0,00E+00 0,00E+00 0,00E+00 0,00E+00 0,00E+00 0,00E+00 0,00E+00 0,00E+00 0,00E+00
Module D -8,95E+02 0,00E+00 -8,95E+02 -1,24E+04 0,00E+00 -1,24E+04 0,00E+00 0,00E+00 0,00E+00 -5,77E+00
LEGEND:
Product stage
End of life stage
Benefits and loads beyond the system boundary
EPR = use of renewable primary energy excluding renewable primary energy resources used as raw materials; RR = use of renewable primary energy resources
used as raw materials; TRR = total use of renewable primary energy resources (EPR + RR); EPNR = use of non-renewable primary energy excluding non-
renewable primary energy resources used as raw materials; RNR = use of non-renewable primary energy resources used as raw materials; TRNR = total use of
non-renewable primary energy resources (EPRN + RNR); MS = use of secondary material; CSR = use of renewable secondary fuels; CSNR = use of non-renewable
secondary fuels.
NOTES:
P.C.I. – Net calorific value
Values expressed by declared unit (1 t of cold-formed welded structural hollow sections).
DAPHabitat System 11
2.5. Other environmental information describing diferente waste categories
Hazardous waste disposed Non-hazardous waste disposed Radioactive waste disposed
Unit kg kg kg
Modules A1-A3 8,83E-01 0,00E+00 0,00E+00
Module C2 ND ND ND
Module C3 ND ND ND
Module C4 0,00E+00 0,00E+00 0,00E+00
Module D ND ND ND
LEGEND:
Product stage
End of life stage
Benefits and loads beyond the system boundary
NOTES:
Values expressed by declared unit (1 t of cold-formed welded structural hollow sections).
The characteristics that make waste hazardous are described in the applicable legislation in force, for example in the European Waste Framework
Directive.
ND – module not declared
2.6. Environmental information describing output flows
Components for re- Materials for Materials for energy
Exported energy
use recycling recovery
Unit kg kg kg MJ
Modules A1-A3 0,00E+00 4,43E+01 0,00E+00 0,00E+00
Module C2 0,00E+00 0,00E+00 0,00E+00 0,00E+00
Module C3 0,00E+00 1,00E+03 0,00E+00 0,00E+00
Module C4 0,00E+00 0,00E+00 0,00E+00 0,00E+00
Module D 0,00E+00 0,00E+00 0,00E+00 0,00E+00
LEGEND:
Product stage
End of life stage
Benefits and loads beyond the system boundary
NOTE:
Values expressed by declared unit (1 t of cold-formed welded structural hollow sections).
12 DAPHabitat System
2.7. Information describing the biogenic carbon content at the factory gate
Biogenic carbon content* Units* Modules A1-A3 (results)
Biogenic carbon content in product kg C -
Biogenic carbon content in accompanying packaging kg C 0,831
* 1 kg biogenic carbon is equivalent to 44/12 kg of CO2.
Values expressed by declared unit (1 t of cold-formed welded structural hollow sections).
3. SCENARIOS AND ADDITIONAL TECHNICAL INFORMATION
3.1. C2 Transport – End of life of the product
Parameter Units Results expressed per declared unit
Vehicle type - Truck 16-32 t, EURO 5
Distance km 300
Average load of the truck t 5,79
3.2. C3 Waste processing for reuse, recovery and/or recycling – End of life of the product
Parameter Units Results expressed per declared unit
Material for re-use kg 0
Material for recycling kg 1 000
Material for energy recovery kg 0
3.3. C4 Disposal – End of life of the product
Parameter Units Results expressed per declared unit
Material for final deposition kg 0
DAPHabitat System 13
3.4. Scenario and technical information for module D
Parameter Units Results expressed per declared unit
Net output flow of steel scrap -
structural hollow sections at the kg 976
end of life
Net output flow of steel scrap -
scrap from the manufacturing kg 42,7
process
Steel avoided production kg 905
Location of end-of-waste point - At the scrap sorting plant.
Steel manufactured from scrap is considered to have the same
Point of functional equivalence -
quality as steel manufactured from primary material.
The net output flow of steel scrap is calculated by the difference
between the flow of steel scrap that will be recycled and the input
flow of steel scrap used in the steel consumed in the manufacturing
Assumptions - of the structural hollow sections. The following specific
consumptions of scrap during steel manufacturing were considered:
1.13 and 1.04 kg scrap / kg steel, for Europe and the rest of the
world, respectively.
3.5. Additional information on release of dangerous substances to indoor air, soil, and water
during the use stage
Not applicable.
14 DAPHabitat System
REFERENCES
✓ General Instructions of the DAPHabitat System, Version 2.0, Edition June 2022 (in www.daphabitat.pt);
✓ PCR – basic model for construction products and services. DAPHabitat System. Version 2.2, June 2022 (in
www.daphabitat.pt);
✓ ISO 14025:2009 Environmental declarations and labels – Type III environmental declarations – Principles and
procedures;
✓ EN 15804:2012+A2:2019 Sustainability of construction works – Environmental product declarations – Core
rules for the product category of construction products;
✓ EN 15942:2021 Sustainability of construction works – Environmental product declarations – Communication
format business-to-business.
DAPHabitat System 15
