Logo of the EPD’s owner]
DAPHabitat System Environmental Product Declaration
www.daphabitat.pt [according to ISO 14025, EN 15804:2012+A2:2019 and EN 15942]
Declaration number: DAP 002:2023
Products SIBExtreme
Issue date: 18/10/2023 Valid until: 17/10/2028
SIB - SOCIEDADE INDUSTRIAL DE BRITAGEM DE PEDRA, LDA.
Versão 1.4. September 2023 Edition
1
Index
1. GENERAL INFORMATION ....................................................................................................................... 1
1.1. The DAPHAbitat System ............................................................................................................................... 1
1.2. EPD owner .................................................................................................................................................... 1
1.3. Information concerning the EPD .................................................................................................................. 2
1.4. Demonstration of the verification ............................................................................................................... 2
1.5. EPD Registration .......................................................................................................................................... 2
(Plataforma para a Construção Sustentável) ............................................................................................................. 2
1.6. PCR (product category rules) basic model ................................................................................................... 3
1.7. Relevant c-PCR (Complementary product category rules) .......................................................................... 3
1.8. Information concerning the product/product class ..................................................................................... 4
1.9. Calculation rules of the LCA ......................................................................................................................... 5
1.10. Use of average environmental performance ............................................................................................... 6
1.11. Technical information for Reference Service Life (RSL) ............................................................................... 6
1.12. Flow diagram of input and output of the processes .................................................................................... 6
2. CORE ENVIRONMENTAL IMPACT INDICATORS ...................................................................................... 8
2.1. Description of the system boundaries ......................................................................................................... 8
2.1.1. Justification for the exemption to declare modules C1, C2, C3, C4 and D .............................................. 9
2.2. Core environmental impact indicators ...................................................................................................... 10
2.3. Additional environmental impact indicators ............................................................................................. 11
2.4. Indicators describing resource use ............................................................................................................ 12
2.5. Other environmental information describing different waste categories ................................................. 13
2.6. Environmental information describing output flows ................................................................................. 13
2.7. Information describing the biogenic carbon content at the factory gate .................................................. 14
3. SCENARIOS AND ADDITIONAL TECHNICAL INFORMATION ................................................................. 14
3.1. A4 Transport to the building site – Construction process stage ................................................................ 14
3.2. Additional information on release of dangerous substances to indoor air, soil, and water during the use
stage 15
4. REFERENCES ......................................................................................................................................... 16
DAPHabitat System
iii
1. GENERAL INFORMATION
1.1. The DAPHAbitat System
Sustainable Construction Platform
Program operator:
www.centrohabitat.net
centrohabitat@centrohabitat.net
Departamento Engenharia Civil
Address: Universidade de Aveiro
3810-193 Aveiro
Email address: deptecnico@centrohabitat.net
Telephone number: (+351) 234 401576
Website:
www.daphabitat.pt
Logo
1.2. EPD owner
Name of the owner: SIB – Sociedade Industrial de Britagem de Pedra, Lda.
Rua São Luis Gonzaga, n.º 50, Padrão
Production site:
2410-199, Leiria, Portugal
Rua São Luis Gonzaga, n.º 50, Padrão
Address (head office):
2410-199, Leiria, Portugal
Telephone: +351 244 744 431
E-mail: geral@sibland.pt
Website: www.sibland.company
Logo:
Information concerning the
applicable management
Systems:
ISO 9001:2015 – Quality Management System
Specific aspects regarding the CAE Principal: 23640-R3
production:
Organization’s environmental SIBLAND carries out sustainable product development with respect for the environment and without
policy: adversely affecting the expectations of future generations.
DAPHabitat System 1
1.3. Information concerning the EPD
Authors: 1. Technological Center of Ceramics and Glass
2. SIB – Sociedade Industrial de Britagem de Pedra, Lda.
Contact of the authors: 1. CTCV materials: habitat | iParque – Parque Tecnológico de Coimbra - Lote 6 | 3040-540 Antanhol –
Portugal
(T) +351 239 499 200
Marisa Almeida: marisa@ctcv.pt
2. SIBLAND – Sociedade Industrial de Britagem de Pedra Lda. Rua São Luis Gonzaga, n.º 50, Padrão
2410-199, Leiria, Portugal
(T) +351 244 744 431
Issue date: 2023-10-18
Registration date: 2023-11-03
Registration number: DAP 002:2023
Valid until: 2028-10-17
Representativity of the EPD
EPD of a decorative mortar for floors, produced in one production unit, belonging to a single producer
(location, manufacturer,
(SIB – Sociedade Industrial de Britagem de Pedra Lda.)
group of manufacturers):
Where to consult explanatory
https://sibland.company/
material:
Type of EPD: EPD from cradle-to-gate with the distribution option (A1-A3, A4)
1.4. Demonstration of the verification
External independent verification, accordingly with the standard ISO 14025:2010 and EN 15804:2012+A2:2019
Certification Body Verifier(s)
(CERTIF – Associação para a Certificação) (Helena Gervásio)
1.5. EPD Registration
Programme Operator
(Plataforma para a Construção Sustentável)
DAPHabitat System 2
1.6. PCR (product category rules) basic model
Name: PCR: Basic module for construction products and services
Issue date: 19/01/2016
Number of registration on the data RCP-mb001
base:
Version: Version 2.3 (August 2023)
Identification and contact of the Marisa Almeida | marisa@ctcv.pt
coordinator (s): Luís Arroja | arroja@ua.pt
José Dinis Silvestre | jose.silvestre@ist.utl.pt
Marisa Almeida | marisa@ctcv.pt
Identification and contact of the
Luís Arroja | arroja@ua.pt
authors: José Silvestre | jds@civil.ist.utl.pt
Fausto Freire
Cristina Rocha
Ana Paula Duarte
Ana Cláudia Dias
Helena Gervásio
Victor Ferreira
Ricardo Mateus
António Baio Dias
Composition of the Sectorial Panel: -
Consultation period: 18/11/2015 - 18/01/2016
Valid until: 01/06/2027
CEN standard EN 15804 serves as the core Product Category Rules (PCR)
1.7. Relevant c-PCR (Complementary product category rules)
Name: Not applicable
Issue date: -
Number of registration on the data -
base:
Version: -
-
Identification and contact of the
coordinator (s):
Identification and contact of the -
authors:
Composition of the Sectorial Panel: -
Consultation period: -
Valid until: -
DAPHabitat System 3
1.8. Information concerning the product/product class
Identification of the SIBEXTREME products
product:
Illustration of the
product:
Brief description of
The Extreme product range combines abilities that make it possible to create truly seamless high-performance
the product:
Terrazzo floors. The SIBExtreme Style product consists in a decorative Terrazzo mortar with high mechanical
strength. The SIBExtreme Flow is a highly resistant self-levelling mortar with a decorative effect. The SIBExtreme
Style, SIBExtreme Loft and SIBExtreme Flow are bi-component products, composed of mortar and a liquid resin.
Products from the SIBExtreme range are classified as high-performance decorative mortars, due to their physical
and mechanical characteristics with a high resistance to abrasion. This performance can be achieved even with
an application with a thickness of 10 mm.
Table 1: Composition of the products
SIBExtreme AF Flow SIBExtreme AF Loft SIBExtreme AG Style
Component A 20kg + 30kg aggregates 20 kg 20 kg
Component B (liquid) 11 kg (9,2 l) 3,4 to 3,6 kg (17 a 19%) 13,6 kg (11 l)
Component C (aggregate) ‒ ‒ 30 kg
Main technical
Table 2: Technical characteristics of the products
characteristics of the
SIBExtreme AF SIBExtreme AF SIBExtreme AG STYLE Norm
product:
Flow LOFT
Density of component B 1,22 ± 0,02 1,22 ± 0,02 1,22 ± 0,02 ‒
Minimum thickness after
10 mm 10 mm 10 mm ‒
sanding
30 to 90 30 to 90
Opening time (22ᵒC) 30 to 90 minutes ‒
minutes minutes
Thickness of application 10 a 20 mm 10 a 20 mm 12 a 22 mm ‒
Between 2 to 5 Between 2 to 5
Open to traffic Between 2 to 5 days ‒
days days
Aggregates < 1 mm 1 to 3 mm ‒ ‒
Shrinkage < 800 µm/m < 800 µm/m < 800 µm/m EN 13454-2
24h: 40 to 80 MPa
28 days: 60 to 28 days: 40 to 7 days: 50 to 90 MPa
Compressive strength EN 13892-2
80 MPa 80 MPa 28 days: 60 to 100
MPa
24h: 9 to 15 MPa
28 days: 20 28 days: 12 to
Flexural strength 7 days: 12 to 16 MPa EN 13892-2
MPa 15 MPa
28 days: 13 to 20 MPa
A3 – A1,5 (Quartz)
Abrasion resistance A3 – A1,5 (Granite)
A12 – A1,5 A3 – A1,5 EN 13892-3
(Böhme test) A12 – A9 (Marble)
A6 – A3 (Basalt)
Description of the Due to its technical performance, the SIBExtreme products can be used in heavy industrial applications and with
product’s the addition of special hard aggregates Extreme it withstands heavy truck traffic, vehicles, etc.
application/use: It is recommended the use of the primer SIBAQUAPOX and the use of the SIBECOFILLER for the filling during the
polishing process.
DAPHabitat System 4
Placing on the Products covered by regulation (EU) No. 305/2011 require a declaration of performance (table 2 above) taking
market / Rules of into account the harmonized European standard regulation or the European technical assessment and the CE
application in the marking.)
market / Technical Harmonized technical specification: EN 13813:2002 Screed material and floor screeds - Screed material –
rules of the product: Properties and requirements
Quality control: Factory Production Control (Aggregates): EN 12620:2002 + A1:2008; EN 13139:2002 + EN 13139:2002/AC:2004
Special delivery
Not applicable
conditions:
Components and Special binders – 5/40%
substances to Filler material – 10/50%
declare: Additives – 0/5%
Aggregates– 10/50%
Where explanatory The raw materials are stored in silos, big bags or bags in the factory and introduced gravimetrically according to
material may be the respective formula and mixed with a controlled and timed speed.
obtained: The mixture is then packaged.
Quality and environmental standards by ISO 9001:2015 and the provisions described in the relevant regulations.
The SIBExtreme product can be found at dealers and professional applicators.
History of the LCA
Not applicable
studies:
1.9. Calculation rules of the LCA
Functional unit: --
Declared unit: 1 kg of decorative mortar for floors
System boundaries: EPD from cradle-to-gate with the distribution stage (A1-A3, A4)
Criteria for the exclusion: The following processes were not considered in this study, since they fell under the cut-off
criteria:
• The environmental loads associated with the construction of industrial infrastructures and
the manufacture of machinery and equipment;
•The environmental loads related to the infrastructures (production of vehicles, road
maintenance) of the transport of pre-products;
Assumption and limitations This EDP is intended to represent one (1) product (and respective ranges) that can be
produced in one (1) manufacturing unit.
Quality and other characteristics about The production data collected corresponds to the year 2021. The generic data used belong
the information used in the LCA: to the Ecoinvent v3.7 databases and comply with the quality criteria (age, geographical and
technological coverage, plausibility, etc.) of generic data.
Allocation rules: In the industrial unit, various powder products are manufactured using the same production
process, however, each product has its specific recipe.
As the company also manufactures aggregates, the breakdown of energy consumption
according to the measurements and indications made by the company were also taken in
consideration.
A mass allocation was considered in the different mortars produced.
Software used for the assessment: SimaPro, version 9.2
Background database used for the LCA: Ecoinvent database version 3.7.1 published in December 2020; approach “cut-off”
Comparability of EPD for construction The EPD of construction products and services cannot be comparable in case they are not
products produced according to EN 15804 and EN 15948 and according to the comparability
conditions determined by ISO 14025.
DAPHabitat System 5
1.10. Use of average environmental performance
This EPD presents the average environmental performance at entire range of SIBExtreme products produced by SIB
in 2021, with the same raw material recipe. The variability of environmental performance between specific
products is not relevant.
1.11. Technical information for Reference Service Life (RSL)
Not applicable. This is a cradle-to-gate EPD with the distribution stage (A4).
1.12. Flow diagram of input and output of the processes
Figure 1: Production Process of the Mortars and Hardeners (PP2) (line 1 left, line 2 right).
Production Process of the Mortar (PP2):
The various raw materials (aggregates, fillers, special binders and additives) are transported in tanker trucks, plastic bags or big-
bags, with quality control carried out on the raw materials upon receipt.
The storage of these raw materials in bulk is done in silos. As for the raw materials in bags or big-bags, it is carried out on racks
to a warehouse with controlled temperature and humidity.
The final powdered product (decorative mortar for floors) is obtained from the mixture of different raw materials, based on a
pre-established formulation/recipe. Raw materials are dosed automatically through scales incorporated in the production lines.
The components after dosing are then discharged to be subjected to mixing and homogenization in a mixer through pneumatic
valves. Mixing time varies depending on the specific composition of the product. After mixing, the product is discharged into
the hopper of the bagging machine.
DAPHabitat System 6
The last stage of the manufacturing process consists of bagging and palletizing the product. The powdered products are
packaged in printed kraft paper bags using electrical equipment and then placed on a wooden pallet. Finally, pallets and bags
are wrapped in stretch film.
Figure 2: Production scheme – inputs and outputs (only applicable to A1, A2, A3 and A4). Excluded from borders the stage of construction, use
and maintenance, demolition and final disposal.
DAPHabitat System 7
2. CORE ENVIRONMENTAL IMPACT INDICATORS
2.1. Description of the system boundaries
(✓= included; ND = module not declared)
BENEFITS AND LOADS
CONSTRUCTION
PRODUCT STAGE USE STAGE END OF LIFE STAGE BEYOND THE SYSTEM
PROCESS STAGE
BOUNDARY
la
y lp p u s la ire ta m w a R tro p s n a rT g n iru tc a fu n a M tro p s n a rT s s e c o rp n o ita lla ts n i n o
itc
u
e s U e c n a n e tn ia M ria p e R tn e m e c a lp e R tn e m h s ib ru fe R e s u y g re n e la n o ita re p O e s u re ta w la n o ita re p O n o itilo m e d ,s n o itc u rts n eo Dc - tro p s n a rT g n is s e c o rp e ts a W la s o p s iD
itn
e ,yt ro ep v og cn eil rc y ,ec ese ur
-
rts R
n
o
C
A1 A2 A3 A4 A5 B1 B2 B3 B4 B5 B6 B7 C1 C2 C3 C4 D
✓ ✓ ✓ ✓ ND ND ND ND ND ND ND ND ND ND ND ND ND
Modules A1-A3 include those processes that provide energy and material input for the system (A1), transport up to the factory gate of the
plant (A2), manufacturing processes (A3) as well as waste processing.
Module A4 includes the transport from the production site to the customer or to the point of installation of the adhesive mortar. One scenario
was considered for the transport: 2000 km (truck).
Module A5 considers all adhesive mortar installation steps and packaging waste processing (recycling, incineration, disposal). Is was not
considered in this study.
Module B1 considers the use of the adhesive/decorative mortar. It was not considered in this study.
Module B2 includes the cleaning of the adhesive mortars. Provision of water, cleaning agent for the cleaning of the adhesive mortars, incl.
wastewater treatment. It was not considered in this study.
Modules B3-B4-B5 are related to the repair, replacement, and refurbishment of adhesive/decorative mortars. If the adhesive mortars are
properly installed no repair, replacement or refurbishment processes are necessary, but modules B3-B4-B5 are not considered according to
EN17160.
Modules B6-B7 consider energy use for operating building integrated technical systems (B6) and operational water use for technical building-
related systems. No operational energy or water use are considered. Cleaning water is declared under B2. It was not considered in this study.
Module C1 refers to the demolition and de-construction process of the adhesive mortars from the building. It was not considered in this study.
Module C2 considers transportation of the discarded adhesive mortars to a recycling or disposal process. It was not considered in this study
Module C3 considers every process (collection, crushing process etc.) properly for recycling the adhesive mortars. It was not considered in this
study
DAPHabitat System 8
Module C4 includes all the landfill disposal processes, including pre-treatment and management of the disposal site it was not considered in
this study.
Module D was not considered in this study.
2.1.1. Justification for the exemption to declare modules C1, C2, C3, C4 and D
Given that this is a product that meets the three criteria defined in point 5.2 of standard EN 15804:2012+A2:2019+AC, namely:
• it is physically integrated with other materials during the application, and physically separated from the rest at the
end of its useful life is not possible;
• not lethal due to end-of-life physical or chemical transformation processes and;
• this product does not contain biogenic carbon
may be exempt from declaring modules C1, C2, C3, C4 and D.
DAPHabitat System 9
2.2. Core environmental impact indicators
Depletion
Global Global warming
Global warming Global warming potential of the
warming potential land use
potential fossil; potential biogenic; stratospheric Acidification
potential total; and land use change;
ozone layer; potential; AP
GWP-fossil GWP-biogenic
GWP-total GWP-luluc
ODP
Unit kg CO2 eq. kg CO2 eq. kg CO2 eq. kg CO2 eq. kg CFC 11 eq. mol H+ eq.
Module A1-A3
2.11E-01 2.39E-01 -2.77E-02 5.09E-04 2.74E-08 9.75E-04
Module Scenario A4.1
A4 2.70E-01 2.70E-01 2.16E-04 2.05E-06 6.27E-08 5.32E-04
LEGEND:
Product stage
Construction process stage (only A4)
Values expressed by declared unit.
Module A4 – Scenario A4.1 - The scenario considered was 2000 km (truck).
Eutrophicati Abiotic Abiotic
Eutroph. Formation
on potential Eutroph. depletion depletion Water (user)
aquatic potential potential potential of potential for potential for deprivation
aquatic tropospheric non-fossil fossil
freshwater; terrestrial; potential;
marine; ozone; resources resources
potential
EP- EP-terrestrial WDP
EP-marine POCP ADP-
freshwater minerals&metals ADP-fossil
m3 World eq.
Units kg P eq. kg N eq. mol N eq. Kg COVNM eq. kg Sb eq. MJ, P.C.I
deprived
Modules A1-A3
7.71E-06 2.17E-04 2.48E-03 7.12E-04 2.63E-07 3.16E+00 6.87E-02
Module Scenario A4.1
A4 1.47E-07 8.87E-05 9.88E-04 3.49E-04 1.15E-08 3.83E+00 -8.11E-04
LEGENDA:
Product stage
Construction process stage (only A4)
Values expressed by declared unit.
Module A4 – Scenario A4.1 - The scenario considered was 2000 km (truck).
DAPHabitat System 10
2.3. Additional environmental impact indicators
Potential
Potential Potential
Human Potential Potential
incidence of Comparative
exposure Comparative Comparative Toxic Potential soil
disease due Toxic Unit for
efficiency Toxic Unit for Unit for humans, quality index
to PM humans, not
relative to ecosystems cancer effects
emissions cancer effects
U235 SQP
ETP-fw HTP-c
PM HTP-nc
IRP
Disease
Unit kBq U 235 eq. CTUe CTUh CTUh -
incidence
Modules A1-A3
1.46E-08 9.35E-03 4.84E+00 7.67E-11 4.61E-09 4.44E+00
Module Scenario A4.1
A4 1.56E-08 1.69E-02 1.53E+00 2.02E-11 2.39E-09 1.22E-02
LEGEND:
Product stage
Construction process stage (only A4)
The impact indicator “POTENTIAL HUMAN EXPOSURE EFFICIENCY RELATIVE TO U235” focuses mainly on the possible impact of a low dose of ionising radiation
on human health resulting from the nuclear fuel cycle. It does not consider effects arising from possible nuclear accidents, occupational exposure or the disposal
of radioactive waste in underground facilities. Potential ionising radiation from soil, radon and some building materials is also not measured by this indicator.
The results of the indicators “POTENTIAL COMPARATIVE TOXIC UNIT FOR ECOSYSTEMS (ETP-FW)”, “POTENTIAL COMPARATIVE TOXIC UNIT FOR HUMANS,
CANCER EFFECTS”, “POTENTIAL COMPARATIVE TOXIC UNIT FOR HUMANS, NOT CANCER EFFECTS” and “POTENTIAL SOIL QUALITY INDEX” should be used with
caution as the uncertainties associated with them are high or there is little experience with the indicator.
Values expressed by declared unit.
Module A4 – Scenario A4.1 - The scenario considered was 2000 km (truck).
DAPHabitat System 11
2.4. Indicators describing resource use
Primary energy
EPR RR TRR EPNR RNR TRNR
Unit MJ, P.C.I. MJ, P.C.I. MJ, P.C.I. MJ, P.C.I. MJ, P.C.I. MJ, P.C.I.
Modules A1-A3
4.24E-01 5.38E-01 9.62E-01 2.71E+00 6.74E-01 3.39E+00
Module Scenario A4.1
A4 5.63E-03 0.00E+00 5.63E-03 4.06E+00 0.00E+00 4.06E+00
LEGEND:
Product stage
Construction process stage (only A4)
EPR = use of renewable primary energy excluding renewable primary energy resources used as raw materials; RR = use of renewable primary energy resources
used as raw materials; TRR = total use of renewable primary energy resources (EPR + RR); EPNR = use of non-renewable primary energy excluding non-
renewable primary energy resources used as raw materials; RNR = use of non-renewable primary energy resources used as raw materials; TRNR = total use of
non-renewable primary energy resources (EPRN + RNR);
Values expressed by declared unit.
Module A4 – Scenario A4.1 - The scenario considered was 2000 km (truck).
Secondary materials and fuels, and use of water
MS CSR CSNR Net use of fresh water
Unit kg MJ, P.C.I. MJ, P.C.I. m3
Modules A1-A3
0.00E+00 0.00E+00 0.00E+00 1.95E-03
Module Scenario A4.1
A4 0.00E+00 0.00E+00 0.00E+00 5.75E-06
LEGEND:
Product stage
Construction process stage (only A4)
MS = use of secondary material; CSR = use of renewable secondary fuels; CSNR = use of non-renewable secondary fuels.
Values expressed by declared unit.
Module A4 – Scenario A4.1 - The scenario considered was 2000 km (truck).
DAPHabitat System 12
2.5. Other environmental information describing different waste categories
Hazardous waste disposed Non-hazardous waste disposed Radioactive waste disposed
Unit kg kg kg
Modules A1-A3
4.35E-06 1.84E-02 1.12E-05
Module Scenario A4.1
A4 1.01E-05 1.60E-04 2.77E-05
LEGEND:
Product stage
Construction process stage (only A4)
The characteristics that make waste hazardous are described in the applicable legislation, for example in the Waste Directive (UE).
Values expressed by declared unit.
Module A4 – Scenario A4.1 - The scenario considered was 2000 km (truck).
2.6. Environmental information describing output flows
Exported energy
Components for Materials for Materials for
re-use recycling energy recovery
Energy carrier 1 … Energy carrier n
Unit kg kg kg MJ MJ MJ
Modules A1-A3
0.00E+00 9.07E-03 3.35E-03 0.00E+00 -- --
Module Scenario A4.1
A4 0.00E+00 0.00E+00 0.00E+00 0.00E+00 -- --
LEGEND:
Product stage
Construction process stage (only A4)
The characteristics that make waste hazardous are described in the applicable legislation, for example in the Waste Directive (UE).
Values expressed by declared unit.
Module A4 – Scenario A4.1 - The scenario considered was 2000 km (truck).
DAPHabitat System 13
2.7. Information describing the biogenic carbon content at the factory gate
Biogenic carbon content* Units** Modules A1-A3 (results)
Biogenic carbon content in product kg C Not applicable
Biogenic carbon content in accompanying packaging kg C Not applicable
* 1 kg biogenic carbon is equivalent to 44/12 kg of CO2.
** This information can be omitted whenever the content of biogenic carbon in the product, or in the respective packaging, is less than 5% of the
mass of the product, or the respective packaging.
The analyzed products do not contain biogenic carbon, except for some materials present in the primary packaging
(paper bags) and secondary packaging (wooden pallets and cardboard boards). Since its weight does not exceed
the limit of 5% concerning the total mass of the product, it is not necessary to declare biogenic carbon, as
indicated in EN 15804:2012+A2+AC.
3. SCENARIOS AND ADDITIONAL TECHNICAL INFORMATION
3.1. A4 Transport to the building site – Construction process stage
Scenario A4.1
Parameter Units*/comments
Name and description of Transport to central
Scenario
the scenario Europe
Name of the scenarios
Related scenario -
linked to this scenario
Fuel type and consumption of
Litre of fuel type per
vehicle or vehicle type used for Road transport by truck
distance, or vehicle
transport e.g. long-distance truck, (16-32 ton class EURO 6)
type**
boat, etc.
Distance km 2000
Capacity utilization (including
% 24ton
empty returns)
Bulk density of transported
kg/m3 1.2
products
Volume capacity utilization factor
(factor: =1 or < 1 or ≥ 1 for
compressed or nested packaged
Not applicable NA
products)
DAPHabitat System 14
3.2. Additional information on release of dangerous substances to indoor air, soil, and water
during the use stage
Volatile Organic Compound (VOC) emission tests were carried out on two products, in accordance with ISO 16000
parts 3, 6, 9 and 11 and CN/TS 16516. The products were fed into emission chambers in order to detect their VOC
emissions after 3 and 28 days of storage in the ventilated chambers, according to the GEV test method
(Gemeinschaft Emissionskontrollierte Verlegewerkstoffe, Klebstoffe und Bauprodukte e.V.). SIBExtreme products
have been proven to meet the requirements for the Emicode EC1RPLUS emission class, such as “very low VOC
emission”.
Parameter (a) Unit Result Additional considerations
COVT after 3 days µg/m3 ≤ 750
COVT after 28 days µg/m3 ≤ 60
COSVT after 28 days µg/m3 ≤ 40
R value based on German AgBB LCI µg/m3
1
(NIK) after 28 days
Product classified as:
Sum of non-assessable VOCs µg/m3 ≤ 40
“EC1 PLUS – very low emission” by GEV
Formaldehyde after 3 days µg/m3 ≤ 50
“VOC emissions and content
Acetaldehyde after 3 days µg/m3 ≤ 50 specifications in LEED EQ credit “Low-
emitting products””
Sum of form- and Acetaldehyde µg/m3 ≤ 0,05
Sum of C1A/C1B volatile after 3 days µg/m3 ≤ 10
Any C1A/C1B volatile after 28 days µg/m3 ≤ 1
Sum COVT + COSVT + COVVT after 28 days µg/m3 ≤ 100
max. 40 SVOC
(a) (According to the horizontal standards on the measurement of the release of regulated hazardous
substances from construction products, using harmonised test methods in accordance with the
provisions of the respective Technical Committees for European product standards, when available.
DAPHabitat System 15
4. REFERENCES
✓ General Instructions of the DAPHabitat System, Version 2.1, Edition August 2023 (in www.daphabitat.pt);
✓ PCR – basic module for construction products and services. DAPHabitat System. Version 2.3, August 2023 (in
www.daphabitat.pt);
✓ ISO 14025:2009 Environmental declarations and labels – Type III environmental declarations – Principles and
procedures;
✓ EN 15804:2012 + A2:2019 Sustainability of construction works – Environmental product declarations – Core
rules for the product category of construction products;
✓ EN 15942:2021 Sustainability of construction works – Environmental product declarations – Communication
format business-to-business.
DAPHabitat System 16
