DAPHabitat System E NVIRONMENTAL P RODUCT D ECLAR ATION
www.daphabitat.pt [ACCORDING TO ISO 14025, EN 15804:2012+A2:2019 AND EN 15942]
Declaration number: DAP 007:2024
POLYMERIC PROFILES FOR WALL AND FLOOR COATINGS
ISSUE DATE: 12-07-2024 VALID UNTIL: 11-07-2029
EPW – Tecnologia de Extrusão, Lda.
Version 1.4. Ed. March 2024
i
INDEX
1. GENERAL INFORMATION ....................................................................................................... 1
1.1. THE DAPHABITAT SYSTEM .......................................................................................................................... 1
1.2. EPD OWNER ............................................................................................................................................. 1
1.3. INFORMATION CONCERNING THE EPD ............................................................................................................ 2
1.4. DEMONSTRATION OF THE VERIFICATION .......................................................................................................... 2
1.5. EPD REGISTRATION ................................................................................................................................... 2
1.6. PCR (PRODUCT CATEGORY RULES) BASIC MODEL ............................................................................................... 3
1.7. RELEVANT C-PCR (COMPLEMENTARY PRODUCT CATEGORY RULES) ........................................................................ 3
1.8. INFORMATION CONCERNING THE PRODUCT/PRODUCT CLASS ................................................................................ 4
1.9. CALCULATION RULES OF THE LCA ................................................................................................................... 5
1.10. USE OF AVERAGE ENVIRONMENTAL PERFORMANCE ............................................................................................ 6
1.11. TECHNICAL INFORMATION FOR REFERENCE SERVICE LIFE (RSL) ............................................................................. 7
1.12. FLOW DIAGRAM OF INPUT AND OUTPUT OF THE PROCESSES ................................................................................. 7
2. CORE ENVIRONMENTAL IMPACT INDICATORS ........................................................................ 8
2.1. DESCRIPTION OF THE SYSTEM BOUNDARIES ......................................................................................... 8
2.1.1. JUSTIFICATION FOR THE EXEMPTION TO DECLARE MODULES C1, C2, C3, C4 AND D .............................. 8
2.2. CORE ENVIRONMENTAL IMPACT INDICATORS .................................................................................................... 9
2.3. ADDITIONAL ENVIRONMENTAL IMPACT INDICATORS ......................................................................................... 10
2.4. INDICATORS DESCRIBING RESOURCE USE ........................................................................................................ 11
2.5. OTHER ENVIRONMENTAL INFORMATION DESCRIBING DIFFERENT WASTE CATEGORIES ............................................... 12
2.6. ENVIRONMENTAL INFORMATION DESCRIBING OUTPUT FLOWS ............................................................................ 12
2.7. INFORMATION DESCRIBING THE BIOGENIC CARBON CONTENT AT THE FACTORY GATE ................................................ 13
3. SCENARIOS AND ADDITIONAL TECHNICAL INFORMATION ..................................................... 13
3.1. A4 TRANSPORT TO THE BUILDING SITE – CONSTRUCTION PROCESS STAGE ............................................................. 13
3.2. C1 DE-CONSTRUCTION, DEMOLITION – END OF LIFE OF THE PRODUCT ............................................... 13
3.3. C2 TRANSPORT – END OF LIFE OF THE PRODUCT ................................................................................. 14
3.4. C3 WASTE PROCESSING FOR REUSE, RECOVERY AND/OR RECYCLING – END OF LIFE OF THE PRODUCT
14
3.5. C4 DISPOSAL – END OF LIFE OF THE PRODUCT .................................................................................... 15
3.6. SCENARIO AND TECHNICAL INFORMATION FOR MODULE D ............................................................... 15
4. REFERENCES ........................................................................................................................ 16
ii
1. GENERAL INFORMATION
1.1. The DAPHAbitat System
Sustainable Construction Platform
Program operator: www.centrohabitat.net
geral@clusterhabitat.pt
Departamento Engenharia Civil
Address: Universidade de Aveiro
3810-193 Aveiro
Email address: deptecnico@clusterhabitat.pt
Telephone number: (+351) 234 401576
Website:
www.daphabitat.pt
Logo
1.2. EPD owner
Name of the owner: EPW — Tecnologia de Extrusão, Lda.
Zona Industrial da Guia, Lotes 6, 7 e 8
Production site:
3105-467 – Guia – Pombal, Portugal
Address (head office): Zona Industrial da Guia, Lotes 6, 7 e 8, 3105-467 – Guia – Pombal, Portugal
Telephone: Eng. Bruno Pita - +351236 951 421
E-mail: brunopita@epw.pt
Website: https://www.epw.pt/en/
Logo:
--
Information concerning the
applicable management
Systems:
Specific aspects regarding Division CPC 36 (Rubber and plastic products), Grupo 369, Class 3691, Subclass 36910: Floor
the production: coverings of plastics, in rolls or in the form of tiles; wall or ceiling coverings of plastics
Organization’s
environmental policy:
DAPHabitat System 1
1.3. Information concerning the EPD
Authors: CERIS - Civil Engineering Research and Innovation for Sustainability
Av. Rovisco Pais | 1049-001 Lisboa
Responsible practitioner(s): José Dinis Silvestre and Marco Frazão Pedroso
Contact of the authors: Phone: +351 218 419709
E-mail: jose.silvestre@tecnico.ulisboa.pt e marco.pedroso@tecnico.ulisboa.pt
Issue date: 12/07/2024
Registration date:
14/10/2024
Registration number:
DAP 007:2024
Valid until:
11/07/2029
Representativity of the EPD
(location, manufacturer, EPD corresponding to the polymeric profiles manufactured at an industrial unit in Guia –
Pombal, Portugal.
group of manufacturers):
Where to consult
-
explanatory material:
Type of EPD: EPD from cradle to gate, including transportation (A4) and end-of-life (C1 to C4) and
module D.
1.4. Demonstration of the verification
External independent verification, accordingly with the standard ISO 14025:2010 and EN 15804:2012+A2:2019
Certification Body Verifier
(CERTIF – Associação para a Certificação) (Helena Gervásio)
1.5. EPD Registration
Programme operator
(Plataforma para a Construção Sustentável)
DAPHabitat System 2
1.6. PCR (product category rules) basic model
Name: -
Issue date: -
Number of registration on the data -
base:
Version: -
Identification and contact of the -
coordinator (s):
-
Identification and contact of the
authors:
Composition of the Sectorial Panel: -
Consultation period: -
Valid until: -
CEN standard EN 15804 serves as the core Product Category Rules (PCR)
1.7. Relevant c-PCR (Complementary product category rules)
1. Product Category Rules (PCR) – Floor coatings – V.1.2 (2014) – V.2.2. EDITION
Name:
JUNE 2022
2. Product Category Rules (PCR) – Wall coatings – V.1.2 (2014) – V.2.2. EDITION
JUNE 2022
1. 10/02/2014
Issue date:
2. 10/02/2014
1. PCR001:2014
Number of registration on the data
base: 2. PCR001:2014
1. Version 2.2
Version:
2. Version 2.2
1. Luís Arroja | arroja@ua.pt
Identification and contact of the
coordinator (s): Marisa Almeida | marisa@ctcv.pt
2. Luís Arroja | arroja@ua.pt
Marisa Almeida | marisa@ctcv.pt
Identification and contact of the
1. Marisa Almeida | marisa@ctcv.pt
authors: Luís Arroja | arroja@ua.pt
Ana Cláudia Dias | acdias@ua.pt
2. Marisa Almeida | marisa@ctcv.pt
Luís Arroja | arroja@ua.pt
Ana Cláudia Dias | acdias@ua.pt
1. RMC – Revestimentos de Mármore Compactos, S.A.; Dominó – Indústrias
Composition of the Sectorial Panel:
Cerâmicas, S.A.; MAS – Manuel Amorim da Silva, Lda.; Sonae Indústria, SGPS,
S.A.; APICER – Associação Portuguesa da Indústria de Cerâmica.
2. RMC – Revestimentos de Mármore Compactos, S.A.; Dominó – Indústrias
Cerâmicas, S.A.; MAS – Manuel Amorim da Silva, Lda.; Sonae Indústria, SGPS,
S.A.; APICER – Associação Portuguesa da Indústria de Cerâmica.
1. 01/08/2013 to 30/11/2013
Consultation period:
2. 01/08/2013 to 30/11/2013
1. 01/06/2027
Valid until:
2. 01/06/2027
DAPHabitat System 3
1.8. Information concerning the product/product class
Identification of the product: This EPD covers the polymeric profiles produced at an industrial unit (Guia – Pombal,
Portugal).
Illustration of the product:
Brief description of the product: The product consists of polymeric base profiles for interior and exterior wall and floor
cladding. These profiles can be produced in different colours, presenting a texture similar
to natural wood. The production of these panels occurs at an industrial unit located in
Guia – Pombal, Portugal.
The product consists of polymeric profiles based on wood (40 to 60%), recycled polymer
base (40 to 60%), and chemical additives of known composition (10 to 20%) and freely
available on the market.
The polymeric profiles for interior and exterior wall and floor cladding are available in
dimensions of 2300/3200 x 157 x 16 mm. Given their characteristics, these profiles are
mainly used for interior and exterior wall and floor cladding, designed to create
comfortable environments, and rehabilitate interior and exterior spaces.
Main technical characteristics of the
The technical datasheets of this product are available at:
product:
https://www.epw.pt/en/downloads-2/. Table 1 presents some of the product
characteristics, and the full list of characteristics can be analysed on the website
previously mentioned.
Table 1: Technical characteristics
DESIGNATION VALUE UNIT
HUMIDITY 0,80 %
WARPING 2 MM/ML
DENSITY 1458 KG/M3
IMPACT RESISTANCE MAX 0,12 MM
VICAT 85,2 ºC
HDT 74 ºC
THERMAL EXPANSION
2,79X10-5 MM/MM ºC
COEFFICIENT
MARKING EN 15534-4 PVC W50 UC3
.
Description of the product’s Given their characteristics, these profiles are primarily used for interior and exterior wall
application/use: and floor cladding, developed to create comfortable environments, and rehabilitate
interior and exterior spaces.
Placing on the market / Rules of • EN 15534-4:2014: Composites made from cellulose-based materials and thermoplastics
application in the market / Technical (usually called wood-polymer composites (WPC) or natural fibre composites (NFC)) - Part
rules of the product: 4: Specifications for decking profiles and tiles;
Quality control: The quality control follows:
• EN 15534-4:2014: Composites made from cellulose-based materials and thermoplastics
(usually called wood-polymer composites (WPC) or natural fibre composites (NFC)) - Part
4: Specifications for decking profiles and tiles;
Special delivery conditions:
-
Components and substances to declare:
The product consists of polymeric profiles based on wood (40 to 60%), recycled polymer
base (40 to 60%), and chemical additives of known composition (10 to 20%), freely
available on the market.
DAPHabitat System 4
Where explanatory material may be
Additional information can be obtained at: https://www.epw.pt/en/downloads-2/.
obtained:
History of the LCA studies:
-
1.9. Calculation rules of the LCA
Functional unit: -
Declared unit: The declared unit adopted for the development of this EPD corresponds to the production
of one ton (1 ton) of facade and ceiling cladding profiles, made of polymeric material (wood
+ polymer + others), with a density of 1.459 kg/m3.
System boundaries: This study follows a "cradle-to-gate" approach, also considering its transportation to the
United Kingdom (A4), modules C1 to C4 (end-of-life stage), and module D (benefits beyond
the system boundary), following EN 15804:2012+A2:2019/AC:2021.
Criteria for the exclusion: The LCA developed includes all available data directly associated with the production
process of the polymeric profiles. However, the following processes were not considered in
this study, as they fall within the cutoff criteria of 1% of renewable and non-renewable
primary energy use and 1% of the total mass input of the unit process where they occur,
with a maximum of 5% of energy and mass use in the considered stages (A1-A3):
- Construction of industrial infrastructure, manufacture, and exchange of equipment and
machinery;
- Impacts of infrastructure (vehicle manufacturing, road maintenance) associated with the
transportation of pre-products and raw materials;
- Water consumption or waste and effluents produced in administrative areas and
laboratories, as they are not directly associated with the production process;
- Transportation of small consumables to the industrial unit;
- Other flows considered negligible in modelling due to their contribution below the cutoff
criteria.
Since the EPD follows a "cradle-to-gate" approach considering modules C1 to C4 and D, all
stages of the product lifecycle after they leave the factory are excluded from the scope of
the study, including distribution, construction stage (installation of the product in
equipment or buildings), and usage processes.
Assumption and limitations -
Quality and other characteristics Specific manufacturer data is referenced for the average production of the year 2022.
about the information used in the During that year, the polymeric profiles were produced in Guia – Pombal, Portugal.
LCA:
Allocation rules: The industrial facility where these polymeric profiles are manufactured also produces other
products, including accessories. Considering this situation, an allocation methodology was
used to determine the inputs and outputs associated with the production of these
polymeric profiles, considering three different colours, as previously presented.
Allocation Procedure for Reuse, Recycling, and Recovery: During the production phase
(extrusion and cutting), there are losses of the mixture and effluents that are recirculated
for reuse in the manufacturing process, in a closed circuit. Benefits associated with the
sending of paper, plastic, and metal for recycling were also accounted for, as well as the
loads and benefits associated with the recovery of energy from the incineration of
"Packaging containing or contaminated by hazardous substances" and "Absorbents, filtering
materials (including oil filters without other specifications), cleaning cloths, and protective
clothing, contaminated by hazardous substances," present in the Integrated Waste
Registration Map (IWRM) under the category of Mixtures of equivalent urban waste. The
benefits in module D associated with energy recovery linked to module C3 end-of-life were
considered.
Co-Product Allocation: In this study associated with the production of polymeric profiles,
there are no co-products produced during the manufacturing process. However, in the same
DAPHabitat System 5
factory, other profiles and accessories are also produced. In this case, the allocation to
determine the inputs and outputs associated only with the production of the profiles under
study was performed considering the information directly provided by the producer
regarding the allocations identified by the company.
Water Consumption: The water used originates from the collection of rainwater, which is
collected and stored in four 30 m3 tanks. The existing water consumption is associated with
cleaning and is recirculated in a closed circuit. A loss due to evaporation of about 1 m3 per
month is considered, and according to the producer, the need to introduce water from the
network is estimated at 15 Liters per ton to compensate for evaporation losses.
Energy Consumption, Consumables, and Internal Transportation: Electricity consumption,
per mass of material produced, was estimated based on the annual consumption of the
industrial unit (including internal transportation and operation, including electric forklifts
and overhead cranes) and its allocation to profile production. A percentage of the total
consumption of the industrial unit was first allocated to the board production line, and then
that percentage of the annual electricity consumption was divided by the annual board
production, with the final value directly attributable identified by the producer.
Regarding the consumption of consumables, no significant flows were considered, as the
values indicated by the manufacturer were below the cutoff thresholds, although the
production and final destination of all waste identified in the Integrated Waste Registry Map
(IWRM) for the year 2022 were considered.
Emissions to Air, Water, and Soil: The profile production process does not produce gas
emissions.
Waste: The production of polymeric profiles, despite resulting in the generation of non-
conforming strips and trimmings, is 100% reintegrated. Considering the total waste
production for the year recorded in the IWRM and the annual production of these profiles,
the amount of waste per profile mass produced was determined.
Liquid Effluents: The main water consumption is associated with cleaning the extrusion and
cutting area. However, the water (mostly originating from rainwater collection) is used in a
closed circuit, including the introduction of network water to compensate for losses due to
evaporation. These effluents are collected in a settling tank, treated, and reused in the
process, in a closed circuit.
Software used for the assessment: SimaPro v9.5.0.2
Background database used for the The databases used have been updated in the last 10 years, mainly in 2023 (Ecoinvent
v3.9.1). Regarding technological coverage, all selected datasets involve average European
LCA:
technology or a specific European country (with particular interest in Portugal, when
available, given the location of the industrial unit). Whenever possible, the most similar
dataset available in the software databases was used, reflecting an average combination of
technologies and consumption from European industries (denoted with the suffix RER). The
preference for using the Ecoinvent database is mainly related to its recognized reliability.
However, for some processes, the most suitable dataset was available in other databases,
namely ELCD, which was used to model transportation when not available in Ecoinvent,
based on Tremove model v2.7b (2009) and EcoTransIT (2011).
Comparability of EPD for construction The EPD of construction products and services cannot be comparable in case they are not
produced according to EN 15804 and EN 15948 and according to the comparability
products
conditions determined by ISO 14025.
1.10. Use of average environmental performance
The present EPD represents the production of polymeric profiles (wood and plastic) at an industrial unit in Pombal
- Portugal. Although the same manufacturing process and procedure are followed, there are different commercial
DAPHabitat System 6
references that may vary in thickness or appearance. However, through their mass (since the declared unit is one
ton), it is possible to calculate the associated impacts.
1.11. Technical information for Reference Service Life (RSL)
NOT APPLICABLE
1.12. Flow diagram of input and output of the processes
Figure 1: Production system considering the production processes involved to obtain the polymeric profiles (flowchart of the processes flow
studied in the LCA analysis conducted for the Pombal site).
DAPHabitat System 7
2. CORE ENVIRONMENTAL IMPACT INDICATORS
2.1. DESCRIPTION OF THE SYSTEM BOUNDARIES
(✓= included; ND = module not declared)
BENEFITS AND LOADS
CONSTRUCTION
PRODUCT STAGE USE STAGE END OF LIFE STAGE BEYOND THE SYSTEM
PROCESS STAGE
BOUNDARY
la
y lp p u s la ire ta m w a R tro p s n a rT g n iru tc a fu n a M tro p s n a rT s s e c o rp n o ita lla ts n i n o itc
u
e s U e c n a n e tn ia M ria p e R tn e m e c a lp e R tn e m h s ib ru fe R e s u y g re n e la n o ita re p O e s u re ta w la n o ita re p O n o itilo m e d ,s n o itc u rts n eo Dc - tro p s n a rT g n is s e c o rp e ts a W la s o p s iD
itn
e to p g n ilc y c e r ,y re v o c e r ,e es u
-
rts R
n
o
C
A1 A2 A3 A4 A5 B1 B2 B3 B4 B5 B6 B7 C1 C2 C3 C4 D
✓ ✓ ✓ ✓ ND ND ND ND ND ND ND ND ✓ ✓ ✓ ✓ ✓
The manufacturing process begins when the raw materials arrive at the industrial unit, where they are stored.
The manufacturing process of the polymeric profiles continues with the execution of mixing the raw materials, in the indicated
proportions (a formulation that is proprietary and patented), to obtain a paste. This paste proceeds to an extruder that molds
the paste and obtains the profiles according to the manufacturing requirements, namely density. Additionally, the obtained
profiles are subject to cutting and adjustment to obtain the necessary dimensions. All these procedures are powered by
electricity, sourced either from the grid or from photovoltaic panels for self-consumption.
Then, the profiles are packaged using plastic film and straps for subsequent dispatch.
The transportation considered here is to an intermediate storage location in the United Kingdom, from where the respective
transports to the clients' work sites will be carried out.
Finally, the impacts associated with the end-of-life stage and the potential benefits associated located outside the system
boundary were considered.
2.1.1. JUSTIFICATION FOR THE EXEMPTION TO DECLARE MODULES C1, C2, C3, C4 AND D
Not applicable.
DAPHabitat System 8
2.2. Core environmental impact indicators
Depletion
Global Global warming
Global warming Global warming potential of the
warming potential land use
potential fossil; potential biogenic; stratospheric Acidification
potential total; and land use change;
ozone layer; potential; AP
GWP-fossil GWP-biogenic
GWP-total GWP-luluc
ODP
Unit kg CO2 eq. kg CO2 eq. kg CO2 eq. kg CO2 eq. kg CFC 11 eq. mol H+ eq.
Modules A1-A3 -2,22E+02 5,03E+02 -7,27E+02 2,02E+00 8,82E-06 2,31E+00
Module A4 4,30E+02 4,29E+02 3,91E-01 2,10E-01 9,39E-06 1,78E+00
Module C1 1,24E+01 1,22E+01 1,76E-01 2,20E-03 2,66E-07 6,11E-02
Module C2 9,55E+00 9,54E+00 8,68E-03 4,66E-03 2,09E-07 3,95E-02
Module C3 1,73E+03 7,10E+02 1,02E+03 1,67E-02 4,46E-06 3,93E-01
Module C4 1,37E+01 1,36E+01 1,22E-01 2,26E-03 2,94E-07 6,47E-02
Module D -5,93E+02 -5,90E+02 -5,20E-01 -2,76E+00 -2,15E-05 -1,60E+00
LEGEND:
Product stage NOTES:
Units expressed by declared unit.
Construction process stage
End - of - life stage
Benefits and loads beyond the system boundary
Eutrophication Abiotic Abiotic
Eutrophication Formation
p ao qt uen att ii ca l potential Eu ptr oo tp eh nic ta iati lo n potential of pod te ep nle tit aio l fn o r pod te ep nle tit aio l fn o r W dea pte rir
v
( au ts ioe nr)
freshwater; aquatic terrestrial; tropospheric non-fossil fossil potential;
marine; ozone; resources resources
potential
EP- EP-terrestrial WDP
EP-marine POCP ADP-
freshwater minerals&metals ADP-fossil
m3 World eq.
Units kg P eq. kg N eq. mol N eq. Kg COVNM eq. kg Sb eq. MJ, P.C.I
deprived
Modules A1-A3 2,09E-02 4,45E-01 4,81E+00 1,73E+00 3,09E-03 8,28E+03 1,76E+02
Module A4 3,46E-03 6,72E-01 7,23E+00 2,60E+00 1,39E-03 6,12E+03 2,50E+01
Module C1 8,09E-05 2,55E-02 2,76E-01 1,03E-01 3,21E-05 2,16E+02 5,01E+02
Module C2 7,68E-05 1,49E-02 1,61E-01 5,78E-02 3,08E-05 1,36E+02 5,55E-01
Module C3 5,83E-04 1,77E-01 1,98E+00 5,22E-01 8,85E-05 1,99E+02 9,35E+00
Module C4 7,90E-05 2,73E-02 2,95E-01 1,12E-01 1,90E-05 2,32E+02 1,02E+00
Module D -7,43E-03 -2,76E-01 -3,11E+00 -1,38E+00 -5,42E-04 -8,61E+03 -1,07E+02
LEGENDA: NOTES: P.C.I. – Net calorific value
Units expressed by declared unit.
Product stage “The results obtained for the indicators “Abiotic depletion potential for non-fossil resources
(ADP-minerals&metals)”, “Abiotic depletion potential for fossil resources potential (ADP-
Construction process stage
fossil)” and “Water (user) deprivation potential (WDP)” should be used with caution since
End - of - life stage the uncertainties associated with them are high or there is little experience with the
indicator.”
Benefits and loads beyond the system boundary
DAPHabitat System 9
2.3. Additional environmental impact indicators
Potential Potential
Potential Potential Potential
incidence of Human Comparative
Comparative Comparative Toxic Potential soil
disease due exposure Toxic Unit for
Toxic Unit for Unit for humans, quality index
to PM efficiency humans, not
ecosystems cancer effects
emissions relative to U235 cancer effects SQP
IRP ETP-fw HTP-c
PM HTP-nc
Disease
Unit kBq U 235 eq. CTUe CTUh CTUh -
incidence
Modules A1-A3 2,41E-05 2,70E+01 1,94E+03 3,80E-07 5,71E-06 8,30E+03
Module A4 3,50E-05 3,07E+00 2,23E+03 1,96E-07 4,31E-06 3,65E+03
Module C1 8,94E-06 4,94E-01 1,29E+02 5,53E-09 7,28E-08 5,01E+02
Module C2 7,79E-07 6,82E-02 4,95E+01 4,36E-09 9,58E-08 8,10E+01
Module C3 2,99E-06 4,55E-01 1,83E+03 3,42E-07 1,36E-06 5,69E+01
Module C4 1,61E-06 2,19E-01 1,49E+02 5,35E-09 6,45E-08 5,70E+02
Module D -6,25E-06 -1,06E+01 -4,34E+02 -1,23E-07 -2,02E-06 -9,11E+02
LEGEND:
Product stage
Construction process stage
End-of-life stage
Benefits and loads beyond the system boundary
NOTES:
Units expressed by declared unit.
The impact indicator “POTENTIAL HUMAN EXPOSURE EFFICIENCY RELATIVE TO U235” focuses mainly on the possible impact of a low dose of ionising
radiation on human health resulting from the nuclear fuel cycle. It does not consider effects arising from possible nuclear accidents, occupational
exposure or the disposal of radioactive waste in underground facilities. Potential ionising radiation from soil, radon and some building materials is also
not measured by this indicator.
The results of the indicators “POTENTIAL COMPARATIVE TOXIC UNIT FOR ECOSYSTEMS (ETP-FW)”, “POTENTIAL COMPARATIVE TOXIC UNIT FOR
HUMANS, CANCER EFFECTS”, “POTENTIAL COMPARATIVE TOXIC UNIT FOR HUMANS, NOT CANCER EFFECTS” and “POTENTIAL SOIL QUALITY INDEX”
should be used with caution as the uncertainties associated with them are high or there is little experience with the indicator.
DAPHabitat System 10
2.4. Indicators describing resource use
Primary energy
EPR RR TRR EPNR RNR TRNR
Unit MJ, P.C.I. MJ, P.C.I. MJ, P.C.I. MJ, P.C.I. MJ, P.C.I. MJ, P.C.I.
Modules A1-A3 3,79E+03 0,00E+00 3,79E+03 8,02E+03 2,53E+02 8,27E+03
Module A4 9,51E+01 0,00E+00 9,51E+01 6,12E+03 0,00E+00 6,12E+03
Module C1 1,99E+01 0,00E+00 1,99E+01 2,17E+02 0,00E+00 2,17E+02
Module C2 2,11E+00 0,00E+00 2,11E+00 1,36E+02 0,00E+00 1,36E+02
Module C3 1,62E+01 0,00E+00 1,62E+01 2,00E+02 0,00E+00 2,00E+02
Module C4 9,25E+00 0,00E+00 9,25E+00 2,32E+02 0,00E+00 2,32E+02
Module D -1,62E+03 0,00E+00 -1,62E+03 -8,61E+03 0,00E+00 -8,61E+03
LEGEND: EPR = use of renewable primary energy excluding renewable primary energy resources
used as raw materials; RR = use of renewable primary energy resources used as raw
Product stage materials; TRR = total use of renewable primary energy resources (EPR + RR); EPNR = use
of non-renewable primary energy excluding non-renewable primary energy resources
Construction process stage used as raw materials; RNR = use of non-renewable primary energy resources used as raw
materials; TRNR = total use of non-renewable primary energy resources (EPRN + RNR);
End-of-life stage
NOTE: Units expressed by declared units.
Benefits and loads beyond the system boundary
Secondary materials and fuels, and use of water
MS CSR CSNR Net use of fresh water
Unit kg MJ, P.C.I. MJ, P.C.I. m3
Modules A1-A3 0,00E+00 0,00E+00 0,00E+00 5,37E+00
Module A4 0,00E+00 0,00E+00 0,00E+00 7,45E-01
Module C1 0,00E+00 0,00E+00 0,00E+00 2,76E-01
Module C2 0,00E+00 0,00E+00 0,00E+00 1,66E-02
Module C3 0,00E+00 0,00E+00 0,00E+00 6,59E-01
Module C4 0,00E+00 0,00E+00 0,00E+00 2,77E-01
Module D 0,00E+00 0,00E+00 0,00E+00 -2,27E+00
LEGEND:
Product stage
Construction process stage
End-of-life stage
Benefits and loads beyond the system boundary
MS = use of secondary material; CSR = use of renewable secondary fuels; CSNR = use of non-renewable secondary fuels.
NOTE: Units expressed by declared units.
DAPHabitat System 11
2.5. Other environmental information describing different waste categories
Hazardous waste disposed Non-hazardous waste disposed Radioactive waste disposed
Unit kg kg kg
Modules A1-A3 3,40E-02 1,51E+02 2,08E-02
Module A4 3,90E-02 2,99E+02 1,99E-03
Module C1 9,80E-04 8,51E+02 2,69E-04
Module C2 8,66E-04 6,65E+00 4,42E-05
Module C3 1,09E-03 1,88E+01 3,14E-04
Module C4 1,08E-03 1,00E+03 1,21E-04
Module D -3,28E-02 -2,05E+01 -7,29E-03
LEGENDA:
NOTES:
Product stage
Units expressed by declared unit.
Construction process stage
End-of-life stage
Benefits and loads beyond the system boundary
2.6. Environmental information describing output flows
Exported energy
Components for Materials for Materials for energy
re-use recycling recovery
Energy carrier 1
Unit kg kg kg MJ
Modules A1-A3 0,00E+00 4,19E+01 6,96E+00 0,00E+00
Module A4 0,00E+00 0,00E+00 0,00E+00 0,00E+00
Module C1 0,00E+00 0,00E+00 0,00E+00 0,00E+00
Module C2 0,00E+00 0,00E+00 0,00E+00 0,00E+00
Module C3 0,00E+00 0,00E+00 8,00E+02 0,00E+00
Module C4 0,00E+00 0,00E+00 0,00E+00 0,00E+00
Module D 0,00E+00 0,00E+00 0,00E+00 4,92E+03
LEGEND:
Product stage NOTES:
Units expressed by declared unit.
Construction process stage
End-of-life stage
Benefits and loads beyond the system boundary
DAPHabitat System 12
2.7. Information describing the biogenic carbon content at the factory gate
Biogenic carbon content* Units** Modules A1-A3 (results)
Biogenic carbon content in product Kg C 210.53
Biogenic carbon content in accompanying packaging Kg C Not applicable
* 1 kg biogenic carbon is equivalent to 44/12 kg of CO2.
** This information can be omitted whenever the content of biogenic carbon in the product, or in the respective packaging, is less than 5% of the
mass of the product, or the respective packaging.
3. SCENARIOS AND ADDITIONAL TECHNICAL INFORMATION
3.1. A4 Transport to the building site – Construction process stage
Results expressed per functional or declared unit
Parameter Units*/comments
Scenario A4.1
Name and description of Transport of the polymeric profiles from the manufacturing unit in Guia
Scenario
the scenario – Pombal to a storage location in Leicester – England.
Name of the scenarios
Related scenario A1 to A3
linked to this scenario
Fuel type and consumption of
Litre of fuel type per Process from Ecoinvent 3 “Transport, freight, lorry 16-32 metric ton,
vehicle or vehicle type used for
distance, or vehicle EURO4 {RER}| transport, freight, lorry 16-32 metric ton, EURO4 | Cut-
transport e.g. long-distance truck,
type** off, S”
boat, etc.
Distance km 2.295
Capacity utilization (including
% 100% returns full
empty returns)
Bulk density of transported
kg/m3 1459
products
Volume capacity utilization factor
(factor: =1 or < 1 or ≥ 1 for
Not applicable NA
compressed or nested packaged
products)
* expressed per declared unit
** Directive 2007/37/EC (European Emission Standard)
3.2. C1 DE-CONSTRUCTION, DEMOLITION – END OF LIFE OF THE PRODUCT
Results expressed per functional or declared unit
Parameter Units/comments
Scenario C1.1
Selective demolition of the polymeric profiles of a
Name and description of
Scenario building, including energy for their removal and emission
the scenario
of particles associated with their removal and handling.
Name of the scenarios
Related scenario C2.1
linked to this scenario
Material collected separately kg 1000
Material collected with mixed
kg -
construction waste
Additional assumptions units as appropriate -
DAPHabitat System 13
3.3. C2 TRANSPORT – END OF LIFE OF THE PRODUCT
Results expressed per functional or declared unit
Parameter Units/comments
Scenario C2.1
Transport of waste from these profiles from the
Name and description of
Scenario demolition site (considered to be in England) to the
the scenario
landfill or energy recovery sites.
Name of the scenarios
Related scenario C1.1, C3.1 e C4.1
linked to this scenario
Fuel type and consumption of Ecoinvent 3 process “Transport, freight, lorry 16-32 metric
Litre of fuel type per
vehicle or vehicle type used for
distance, or vehicle ton, EURO4 {RER}| transport, freight, lorry 16-32 metric
transport e.g. long-distance truck,
boat, etc. type* ton, EURO4 | Cut-off, S”
Distance km Avg 30 km
Capacity utilization (including
% 100% considering empty return
empty returns)
Bulk density of transported
kg/m3 NA
products
Volume capacity utilization factor
(factor: =1 or < 1 or ≥ 1 for
Not applicable NA
compressed or nested packaged
products)
Additional assumptions units as appropriate -
*Commission Directive 2007/37/EC (European Emission Standard)
3.4. C3 WASTE PROCESSING FOR REUSE, RECOVERY AND/OR RECYCLING – END OF LIFE OF
THE PRODUCT
Results expressed per functional or declared unit
Parameter Units/comments
Scenario C3.1
Processing of waste for energy recovery, for the case of
Name and description of
Scenario 80% of the waste from these polymeric profiles,
the scenario
considering a location in England.
Name of the scenarios
Related scenario C2.1 and D.1
linked to this scenario
Material for re-use kg -
Material for recycling kg -
Material for energy recovery kg 800 (considering 50% wood and 50% plastic, by mass)
Additional assumptions units as appropriate -
DAPHabitat System 14
3.5. C4 DISPOSAL – END OF LIFE OF THE PRODUCT
Results expressed per functional or declared unit
Parameter Units/comments
Scenario C3.1
Name and description of Processing of waste for landfill, considering 20% of the
Scenario
the scenario waste from these polymeric profiles, in England.
Name of the scenarios
Related scenario C2.1
linked to this scenario
Material for final deposition kg 200 (considering 50% wood and 50% plastic, by mass)
Additional assumptions units as appropriate -
3.6. SCENARIO AND TECHNICAL INFORMATION FOR MODULE D
Results expressed per functional or declared unit
Parameter Units/comments
Scenario D.1
Benefit of energy recovery in module C3, for the case of 80% of the waste
Name and description of
Scenario from polymeric profiles for a location in England that supports such
the scenario
interventions.
Name of the scenarios
Related scenario C3.1
linked to this scenario
Net output flow specified per
units as appropriate 800
material
Avoid production units as appropriate Electricity -2.43 MJ/kg, and heat production -4.89 MJ/kg
Location of end-of-waste point Not applicable -
Point of functional equivalence Not applicable -
Assumptions units as appropriate -
DAPHabitat System 15
4. REFERENCES
✓ General Instructions of the DAPHabitat System, Version 2.1, Edition August 2023 (in www.daphabitat.pt);
✓ PCR – basic module for construction products and services. DAPHabitat System. Version 2.3, August 2023 (in
www.daphabitat.pt);
✓ ISO 14025:2009 Environmental declarations and labels – Type III environmental declarations – Principles and
procedures;
✓ EN 15804:2012 + A2:2019 Sustainability of construction works – Environmental product declarations – Core
rules for the product category of construction products;
✓ EN 15942:2021 Sustainability of construction works – Environmental product declarations – Communication
format business-to-business.
DAPHabitat System 16
