DAPH ABITAT S YSTEM E NVIRONMENTAL P RODUCT D ECLARATION
WWW.DAPHABITAT.PT [ACCORDING TO ISO 14025, EN 15804:2012+A2:2019 AND EN 15942]
Declaration number: DAP 006:2024
SECOLITE® CEMENT BOARD
ISSUE DATE: 10/07/2024 VALID UNTIL: 09/07/2029
PLACACEM, LDA.
Version 1.4.1 Ed. March 2024
SISTEMA DAPHABITAT i
INDEX
1. GENERAL INFORMATION ....................................................................................................... 1
1.1. THE DAPHABITAT SYSTEM .......................................................................................................................... 1
1.2. EPD OWNER ............................................................................................................................................. 1
1.3. INFORMATION CONCERNING THE EPD ............................................................................................................ 2
1.4. DEMONSTRATION OF THE VERIFICATION .......................................................................................................... 2
(PLATAFORMA PARA A CONSTRUÇÃO SUSTENTÁVEL) ...................................................................................................... 2
1.5. EPD REGISTRATION ................................................................................................................................... 2
1.6. PCR (PRODUCT CATEGORY RULES) BASIC MODEL ............................................................................................... 3
1.7. RELEVANT C-PCR (COMPLEMENTARY PRODUCT CATEGORY RULES) ........................................................................ 3
1.8. INFORMATION CONCERNING THE PRODUCT/PRODUCT CLASS ................................................................................ 4
1.9. CALCULATION RULES OF THE LCA ................................................................................................................... 5
1.10. USE OF AVERAGE ENVIRONMENTAL PERFORMANCE ............................................................................................ 6
1.11. TECHNICAL INFORMATION FOR REFERENCE SERVICE LIFE (RSL) ............................................................................. 6
1.12. FLOW DIAGRAM OF INPUT AND OUTPUT OF THE PROCESSES ................................................................................. 7
2. CORE ENVIRONMENTAL IMPACT INDICATORS ........................................................................ 9
2.1. DESCRIPTION OF THE SYSTEM BOUNDARIES ......................................................................................... 9
2.1.1. JUSTIFICATION FOR THE EXEMPTION TO DECLARE MODULES C1, C2, C3, C4 AND D .............................. 9
2.2. CORE ENVIRONMENTAL IMPACT INDICATORS .................................................................................................. 10
2.3. ADDITIONAL ENVIRONMENTAL IMPACT INDICATORS ......................................................................................... 11
2.4. INDICATORS DESCRIBING RESOURCE USE ........................................................................................................ 12
2.5. OTHER ENVIRONMENTAL INFORMATION DESCRIBING DIFFERENT WASTE CATEGORIES ............................................... 13
2.6. ENVIRONMENTAL INFORMATION DESCRIBING OUTPUT FLOWS ............................................................................ 14
2.7. INFORMATION DESCRIBING THE BIOGENIC CARBON CONTENT AT THE FACTORY GATE ................................................ 14
3. SCENARIOS AND ADDITIONAL TECHNICAL INFORMATION ..................................................... 14
3.1. C1 DE-CONSTRUCTION, DEMOLITION – END OF LIFE OF THE PRODUCT .................................................................. 14
3.2. C2 TRANSPORT – END OF LIFE OF THE PRODUCT .............................................................................................. 15
3.3. C3 WASTE PROCESSING FOR REUSE, RECOVERY AND/OR RECYCLING – END OF LIFE OF THE PRODUCT ........................... 15
3.4. C4 DISPOSAL – END OF LIFE OF THE PRODUCT ................................................................................................. 15
3.5. SCENARIO AND TECHNICAL INFORMATION FOR MODULE D ................................................................................. 15
3.6. ADDITIONAL INFORMATION ON RELEASE OF DANGEROUS SUBSTANCES TO INDOOR AIR, SOIL, AND WATER DURING THE USE
STAGE 15
4. REFERENCES ........................................................................................................................ 16
SISTEMA DAPHABITAT ii
1. GENERAL INFORMATION
1.1. The DAPHAbitat System
Sustainable Construction Platform
Program operator: www.centrohabitat.net
centrohabitat@centrohabitat.net
Departamento Engenharia Civil
Address: Universidade de Aveiro
3810-193 Aveiro
Email address: deptecnico@centrohabitat.net
Telephone number: (+351) 234 401576
Website:
www.daphabitat.pt
Logo:
1.2. EPD owner
Name of the owner: PLACACEM, Lda.
Production site: Zona Industrial de Vagos, Lote 50 e 52, 3840-385, Vagos, Portugal
Address (head office): Zona Industrial de Vagos, Lote 50 e 52, 3840-385, Vagos, Portugal
Telephone: +351 234109346
E-mail: geral@secolite.eu
Website: https://secolite.eu/en
Logo:
Information concerning the
Quality Management System (NP EN ISO 9001:2015)
applicable management
Environmental Management System (NP EN ISO 14001:2015)
Systems:
Specific aspects regarding
EN 12467:2012+A2:2018 - Fibre-cement flat sheets. Product specification and test methods
the production:
PLACACEM, Lda:
VISION: To be the leading provider of innovative cement board solutions.
MISSION: We offer our customers high-quality, durable and easy-to-use cement board systems that
meet their most challenging applications.
VALUES: Quality; Sustainability; Innovation; Commitment to customers and employees.
QUALITY AND ENVIRONMENT POLICY
Organization’s PLACACEM LDA's policy aims to promote excellence in its activities, particularly in the manufacture and
sale of cement boards, which includes the following items:
environmental policy:
•Commitment to complying with legislation and all applicable regulatory requirements.
•Personalized attention to the Customer and commitment to meeting their requirements, promoting
their satisfaction.
•Professional and personal development of employees, as well as a spirit of teamwork.
•Raising awareness and training employees to ensure quality in the tasks they perform.
•Commitment to high quality and the continuous improvement of the Quality Management System
through the establishment and review of principles, objectives, targets, systematic evaluation, and the
DAPHabitat System 1
adaptation to the context of the organization of the interested parties and the risks and opportunities
inherent in its activity, improving the production process and the organization's processes.
•Complying with environmental legal requirements and other relevant requirements.
•Commitment to the continuous improvement of the environmental management system to
guarantee sustainable development and the preservation of the environment.
•Adopt the necessary measures to prevent environmental risks.
•Communicate to suppliers and partners, customers and consumers all the principles by which
PLACACEM LDA is governed to contribute to global environmental awareness.
1.3. Information concerning the EPD
Authors: EcoLab - Laboratório de Física e Tecnologia das
Construções da Universidade do Minho
Ricardo Mateus e Cláudia Jacinto
Contact of the authors: Campus de Azurém, Alameda da Universidade, 4800-058 Guimarães
e-mail: ecolab@civil.uminho.pt
Issue date: 10/07/2024
Registration date: 29/07/2024
Registration number: DAP 006:2024
Valid until: 09/07/2029
Representativity of the EPD
(location, manufacturer, EPD of SECOLITE® cement board (Portland Cement Lightweight Boards) produced by one (1) industrial
unit belonging to one (1) producer (PLACACEM Lda).
group of manufacturers):
Where to consult
https://secolite.eu/en
explanatory material:
Type of EPD: EPD from cradle-to-gate with modules C and D (A1-A3, C1-C4 e D)
1.4. Demonstration of the verification
External independent verification, accordingly with the standard ISO 14025:2010 and EN 15804:2012+A2:2019
Certification Body Verifier
(CERTIF – Associação para a Certificação) (Ana Cláudia Dias)
1.5. EPD Registration
Programme operator
(Plataforma para a Construção Sustentável)
DAPHabitat System 2
1.6. PCR (product category rules) basic model
Name: PCR: Basic module for construction products and services
Issue date: Edition August 2023
Number of registration on the data RCP-mb001
base:
Version: Version 2.3
Identification and contact of the Marisa Almeida | marisa@ctcv.pt
coordinator (s): Luís Arroja | arroja@ua.pt
José Dinis Silvestre | jose.silvestre@ist.utl.pt
Marisa Almeida | marisa@ctcv.pt
Identification and contact of the
Luís Arroja | arroja@ua.pt
authors: José Silvestre | jds@civil.ist.utl.pt
Fausto Freire
Cristina Rocha
Ana Paula Duarte
Ana Cláudia Dias
Helena Gervásio
Victor Ferreira
Ricardo Mateus
António Baio Dias
Composition of the Sectorial Panel: -
Consultation period: 18/11/2015 - 18/01/2016
Valid until: 01/06/2027
CEN standard EN 15804 serves as the core Product Category Rules (PCR)
1.7. Relevant c-PCR (Complementary product category rules)
Name: PCR: Wall covering
Issue date: June 2022
Number of registration on the data RCP002:2014
base:
Version: Version 1.2
Identification and contact of the Luís Arroja | arroja@ua.pt
coordinator (s):
Marisa Almeida | marisa@ctcv.pt
Identification and contact of the Ana Cláudia Dias
authors:
Luís Arroja | arroja@ua.pt
Marisa Almeida | marisa@ctcv.pt
Composition of the Sectorial Panel: RMC - Revestimentos de Mármores Compactos, SA
Dominó - Indústrias Cerâmicas, SA
Sonae Indústrias, SGPS
APICER - Associação Portuguesa da Indústria de Cerâmica
Consultation period: 12/08/2013 - 30/11/2013
Valid until: 01/06/2027
DAPHabitat System 3
1.8. Information concerning the product/product class
Identification of the product: SECOLITE® Cement Board
Illustration of the product:
Brief description of the product: SECOLITE® is a lightweight Portland cement and aggregate board, reinforced on both sides
with a glass fibre mesh. The longitudinal edges are formed, and the transverse edges are
cut. They are suitable for the most demanding environments and can be used in the
construction of ceilings, walls, and exterior and interior partitions.
SECOLITE® Cement Boards can be installed vertically or horizontally in steel or wooden
structures and are easily cut with a stylus and fixed to the profiles with screws. They can
also be finished directly and used as a support for tiles, plaster, paint or ETICS systems.
Main technical characteristics of the Table 1: Technical characteristics of the product
product:
Essential Features Performance Harmonized Standard
Classification Type NT/Category B Class I EN 12467:2012+A2:2018
Nominal Thickness
± 10% about Nominal EN 12467:2012+A2:2018
Tolerance
± 0.3% about Nominal,
Nominal Width Tolerance EN 12467:2012+A2:2018
Level I
Nominal Length
± 5 mm, Level I EN 12467:2012+A2:2018
Tolerance
Bordos' Straightness ≤ 0.1%, Level I EN 12467:2012+A2:2018
Bulk Density ≤ 4 mm/m, Level II EN 12467:2012+A2:2018
Moisture Content 10% EN 322
Impermeability to water Impermeable EN 12467:2012+A2:2018
Dimensional Stability
(Length)
ẟI65.85=0.01%, ẟI65.30=-0.03% EN 318
Dimensional Stability
(Thickness)
ẟI65.85=0.1%, ẟt65.30=-0.1% EN 318
Flexural Strength (MOR) >4MPa EN 12467:2012+A2:2018
fc,0,k=2.28MPa (parallel)
Compressive Strength fc,90,k=2.32MPa EN 789
(perpendicular)
Freeze-Freeze Resistance Passes, 25 cycles, RL=0.93 EN 12467:2012+A2:2018
Hot Water Resistance Passes, RL= 0.76 EN 12467:2012+A2:2018
Resistance to immersion-
drying
Passes, 25 cycles RL=0.84 EN 12467:2012+A2:2018
Resistance to Heat-Rain Passes, 25 cycles EN 12467:2012+A2:2018
Reaction to Fire A1 Non-Combustible EN 13501
Steam Transmission µ=40.9 EN ISO 12572
Thermal Conductivity 0.223 W/m.ºC EN 12664
Fungal Resistance 10 – No Growth -
Table 2: Information on basic physical and chemical properties
Physical state Solid
Colour Brownish grey
Odor Odourless
Melting point > 1200 ⁰C
DAPHabitat System 4
Flammability Non-flammable
Solubility Insoluble in water
Apparent density 1000 - 1200 kg/m3
Description of the product’s SECOLITE® Cement Board is intended to be used for the non-structural cladding of
application/use: interior and exterior walls, for the manufacture of floor construction elements, for
structural applications for wall cladding and for the reinforcement of walls, ceilings and
roof truss structures with wooden or steel structure.
SECOLITE® Cement Board can be fixed to wooden or metal structures. The profiles must
be securely fixed to the structure using suitable fixings. Depending on the loads applied to
the board and the additional support, reinforcements between profiles may be required.
Placing on the market / Rules of CE marking (Regulation No 305/2011)
application in the market / Technical EN 12467:2012 +A2:2018 - Flat fibre cement boards. Product specifications and test
rules of the product: methods
EN 13501-1:2018 - Fire resistance of construction materials and elements
Quality control: Certification in the standard for Quality Management Systems, NP EN ISO 9001:2015,
guaranteeing compliance for quality control in production within the industrial unit.
Special delivery conditions: SECOLITE® cement boards are shipped on pallets whose units vary according to their size
(for example, 2400x1200x12.5 boards are shipped on pallets of 36 boards). A forklift with
a capacity of 2 tonnes is recommended and it must be checked that the storage areas can
support the weight of the pallets (1500kg/pallet). The pallets should be stacked with care
to ensure their stability, not more than six high.
Components and substances to declare: The product in question is the result of a mixture of different substances. SECOLITE®
cement boards are made from Portland cement, inorganic aggregates and reinforced with
glass fibre. These substances are not considered dangerous.
Table 3: Components and chemical substances
Name of the REACH
Composition (%) Nº CAS
substance Registration Nº
Portland cement,
inorganic
Portland cement aggregates and 65997-15-1 Not suitable
glass fibre
reinforcements
This product contains no potentially hazardous candidate substances listed in Regulation
(EC) No 1907/2006 (REACH), art. 59, in concentrations greater than 0.1%.
Where explanatory material may be
The information can be found at the following link:
obtained: https://secolite.eu/en/products/secolite-cement-board
History of the LCA studies:
Not applicable.
1.9. Calculation rules of the LCA
Functional unit: --
Declared unit: 1 tonne (1000 kg) of SECOLITE® Cement Boards.
The product can be commercialised in different sizes. Since the production process is the
same, regardless of the thickness or format of the products, it is possible to convert the
results of this EPD to other units such as, for example, m2, multiplying these results by the
conversion factors presented in Table 4.
Table 4: Conversion factors from results to product area (m2).
Thickness (mm) Conversion factor
15 1.65E-02
12.5 1.38E-02
9 9.90E-03
8 8.80E-03
System boundaries: EPD from cradle-to-gate with modules C and D (A1-A3, C1-C4 e D)
DAPHabitat System 5
Criteria for the exclusion: According to EN 15804:2012+A2:2019, the exclusion criterion for unit processes is 1% of the
total energy consumed and 1% of the total mass of the inputs, with special attention paid to
not exceeding a total of 5% of energy and mass flows excluded at each stage of the LCA. In
the case of this EPD, all known flows were included since the company provided all the
information. However, the following processes were not considered in this study:
•Environmental loads from the construction of industrial infrastructure, manufacture, and
exchange of equipment and machinery;
•Infrastructure environmental loads (vehicle manufacturing, road maintenance) associated
with the transport of pre-products and raw materials;
•Environmental loads relating to consumables or waste produced in administrative areas
and laboratories, as they are not directly associated with the production process;
•Environmental loads related to the packaging materials of the raw materials, since the
company uses silos for storing most of the raw materials.
Assumption and limitations The data collected, the results of the environmental impacts and other indicators presented
in this EPD refer to the production period from July 2022 to June 2023 of a product
(SECOLITE® Cement Boards) that can be produced in one (1) industrial unit (Placacem).
Quality and other characteristics All primary process data (controlled by the manufacturer at the factory) was collected at the
about the information used in the factory based on Placacem's internal records. Consumption data was validated with global
consumption invoices and unit control balances, and its quality and representativeness were
LCA:
verified.
The processes in the Ecoinvent v3.9.1 database were used as a support basis for the
construction of the inventory for this study. The processes considered to produce electricity
and natural gas consumed during the production of the SECOLITE® board were modified and
updated to better fit the national reality. Additionally, for some materials, data were
obtained from the literature. Overall, data quality is considered good.
Allocation rules: The factory where SECOLITE® Cement Board is produced does not produce other products.
Therefore, using a methodology to allocate consumption and emissions associated with the
product under study was unnecessary.
Software used for the assessment: SimaPro, version 9.5.0.0.
Background database used for the Ecoinvent Database v3.9.1 – Ecoinvent
LCA:
Comparability of EPD for construction The EPD of construction products and services cannot be comparable in case they are not
products produced according to EN 15804 and EN 15948 and according to the comparability
conditions determined by ISO 14025.
1.10. Use of average environmental performance
Not applicable.
1.11. Technical information for Reference Service Life (RSL)
Not applicable, as this EPD does not include the use stage (module B).
DAPHabitat System 6
1.12. Flow diagram of input and output of the processes
Figure 1: Activities related to the SECOLITE® cement board associated with each life cycle stage.
DAPHabitat System 7
Detailed description of the stages:
1. Supply
The production process for SECOLITE® Cement Boards begins with the acquisition of raw materials. These are
purchased according to production estimates, received, and stored in silos or in the factory's internal warehouse.
2. Measurement and input of additives
Based on production requirements, the additives to be used in the manufacturing process are calculated and
dosed for the mix.
3. Mixing
All the solid and liquid materials are then fed into the electric mixer to form a homogeneous concrete paste.
4. Moulding
The concrete paste and the fibreglass mesh are poured into a continuous line where the cement board is
manufactured.
5. Cutting and stacking
The next stage involves cutting and stacking the boards on pallets according to the length requested in the
production plan (from 2000cm to 3000cm).
6. Storage
In the storage phase, the pallets are placed in towers in the factory's internal warehouse, where the boards
undergo a controlled curing process.
7. Packaging
The material is separated for painting and packaging according to the output plan. The edges of the boards are
painted, and they are packed onto pallets.
8. Dispatch
According to the orders received, the labels are affixed, and the material is loaded onto heavy goods vehicles for
despatch to customers.
DAPHabitat System 8
2. CORE ENVIRONMENTAL IMPACT INDICATORS
2.1. DESCRIPTION OF THE SYSTEM BOUNDARIES
(✓= included; ND = module not declared)
BENEFITS AND
PRODUCT CONSTRUCTION LOADS BEYOND
USE STAGE END OF LIFE STAGE
STAGE PROCESS STAGE THE SYSTEM
BOUNDARY
la
y lp p u s la ire ta m w a R tro p s n a rT g n iru tc a fu n a M tro p s n a rT s s e c o rp n o ita lla ts n i n o itc
u
e s U e c n a n e tn ia M ria p e R tn e m e c a lp e R tn e m h s ib ru fe R e s u y g re n e la n o ita re p O e s u re ta w la n o ita re p O n o itilo m e d ,s n o itc u rts n eo Dc - tro p s n a rT g n is s e c o rp e ts a W la s o p s iD
itn
e to p g n ilc y c e r ,y re v o c e r ,e es u
-
rts R
n
o
C
A1 A2 A3 A4 A5 B1 B2 B3 B4 B5 B6 B7 C1 C2 C3 C4 D
✓ ✓ ✓ ND ND ND ND ND ND ND ND ND ✓ ✓ ✓ ✓ ✓
Modules A1-A3 include the processes that supply energy and material inputs to the system (A1), transport to the factory gate
(A2) and the manufacturing, packaging and waste processing processes during the production phase (A3).
The construction stage (modules A4-A5) and the use stage (modules B1-B7) were not considered in this assessment and are
excluded from the system boundaries.
Module C1 refers to the process of demolition and deconstruction of SECOLITE® Cement Boards.
Module C2 considers the transport of discarded SECOLITE® Cement Boards to a recycling process or landfill.
Module C3 considers all waste processing processes (treatment, crushing, etc.) that are suitable for recycling cement boards.
Module C4 includes all landfill processes, including pre-treatment and landfill site management.
Module D includes the benefits or burdens on the environment generated by reusable products, recyclable materials and/or
energy flows leaving the system under analysis.
2.1.1. JUSTIFICATION FOR THE EXEMPTION TO DECLARE MODULES C1, C2, C3, C4 AND D
Not applicable.
DAPHabitat System 9
2.2. Core environmental impact indicators
Depletion
Global Global warming
Global warming Global warming potential of the
warming potential land use
potential fossil; potential biogenic; stratospheric Acidification
potential total; and land use change;
ozone layer; potential; AP
GWP-fossil GWP-biogenic
GWP-total GWP-luluc
ODP
Unit kg CO2 eq. kg CO2 eq. kg CO2 eq. kg CO2 eq. kg CFC 11 eq. mol H+ eq.
Modules A1-A3 5.34E+02 5.58E+02 -2.41E+01 4.38E-01 1.33E-05 2.45E+00
Module C1 0.00E+00 0.00E+00 0.00E+00 0.00E+00 0.00E+00 0.00E+00
Module C2 3.77E+00 3.77E+00 3.41E-03 1.83E-03 8.19E-08 1.23E-02
Module C3 9.65E+00 9.60E+00 4.40E-02 4.68E-03 1.73E-07 7.86E-02
Module C4 4.17E+00 4.16E+00 3.03E-03 4.75E-03 9.06E-08 3.15E-02
Module D -2.56E+00 -2.47E+00 -9.54E-02 -1.82E-03 -4.07E-08 -2.04E-02
LEGEND:
Product stage
End - of - life stage
Benefits and loads beyond the system boundary
NOTES:
Values expressed by declared unit (1 t of SECOLITE® boards).
Eutrophication Abiotic Abiotic
Eutrophication Formation
p ao qt uen att ii ca l potential Eu ptr oo tp eh nic ta iati lo n potential of pod te ep nle tit aio l fn o r pod te ep nle tit aio l fn o r W dea pte rir
v
( au ts ioe nr)
freshwater; aquatic terrestrial; tropospheric non-fossil fossil potential;
marine; ozone; resources resources
potential
EP- EP-terrestrial WDP
EP-marine POCP ADP-
freshwater minerals&metals ADP-fossil
m3 World eq.
Units kg P eq. kg N eq. mol N eq. Kg COVNM eq. kg Sb eq. MJ, P.C.I
deprived
Modules A1-A3 9.00E-02 5.13E-01 5.65E+00 1.90E+00 7.64E-03 4.98E+03 4.87E+02
Module C1 0.00E+00 0.00E+00 0.00E+00 0.00E+00 0.00E+00 0.00E+00 0.00E+00
Module C2 2.63E-04 4.22E-03 4.46E-02 1.83E-02 1.21E-05 5.34E+01 2.18E-01
Module C3 1.57E-03 3.35E-02 3.62E-01 1.10E-01 1.96E-05 1.48E+02 1.80E+00
Module C4 3.00E-04 1.31E-02 1.41E-01 4.53E-02 6.10E-06 7.69E+01 2.13E+00
Module D -5.31E-04 -6.04E-03 -8.08E-02 -2.06E-02 -3.42E-05 -3.68E+01 -6.10E-01
LEGENDA:
“The results obtained for the indicators “Abiotic depletion potential for non-fossil
Product stage resources (ADP-minerals&metals)”, “Abiotic depletion potential for fossil
End - of - life stage resources potential (ADP-fossil)” and “Water (user) deprivation potential (WDP)”
should be used with caution since the uncertainties associated with them are high
Benefits and loads beyond the system boundary or there is little experience with the indicator.”
NOTES: Values expressed by declared unit (1 t of SECOLITE® boards).
DAPHabitat System 10
2.3. Additional environmental impact indicators
Potential Potential
Potential Potential Potential
incidence of Human Comparative
Comparative Comparative Toxic Potential soil
disease due exposure Toxic Unit for
Toxic Unit for Unit for humans, quality index
to PM efficiency humans, not
ecosystems cancer effects
emissions relative to U235 cancer effects SQP
IRP ETP-fw HTP-c
PM HTP-nc
Disease
Unit kBq U 235 eq. CTUe CTUh CTUh -
incidence
Modules A1-A3 2.28E-05 3.11E+01 2.45E+03 3.11E-07 7.67E-06 1.47E+06
Module C1 0.00E+00 0.00E+00 0.00E+00 0.00E+00 0.00E+00 0.00E+00
Module C2 3.00E-07 7.14E-02 2.63E+01 1.71E-09 3.76E-08 3.18E+01
Module C3 1.24E-05 7.10E-01 6.30E+01 4.09E-09 5.05E-08 1.01E+02
Module C4 2.98E-06 5.47E-02 4.00E+01 1.79E-09 2.38E-08 1.02E+02
Module D -4.48E-07 -6.12E-01 -1.78E+01 -4.80E-09 -3.98E-08 -7.26E+01
LEGEND:
Product stage
End-of-life stage
Benefits and loads beyond the system boundary
NOTES:
Values expressed by declared unit (1 t of SECOLITE® boards).
The impact indicator “POTENTIAL HUMAN EXPOSURE EFFICIENCY RELATIVE TO U235” focuses mainly on the possible impact of a low dose of ionising
radiation on human health resulting from the nuclear fuel cycle. It does not consider effects arising from possible nuclear accidents, occupational
exposure or the disposal of radioactive waste in underground facilities. Potential ionising radiation from soil, radon and some building materials is also
not measured by this indicator.
The results of the indicators “POTENTIAL COMPARATIVE TOXIC UNIT FOR ECOSYSTEMS (ETP-FW)”, “POTENTIAL COMPARATIVE TOXIC UNIT FOR
HUMANS, CANCER EFFECTS”, “POTENTIAL COMPARATIVE TOXIC UNIT FOR HUMANS, NOT CANCER EFFECTS” and “POTENTIAL SOIL QUALITY INDEX”
should be used with caution as the uncertainties associated with them are high or there is little experience with the indicator.
DAPHabitat System 11
2.4. Indicators describing resource use
Primary energy
EPR RR TRR EPNR RNR TRNR
Unit MJ, P.C.I. MJ, P.C.I. MJ, P.C.I. MJ, P.C.I. MJ, P.C.I. MJ, P.C.I.
Modules A1-A3 5.81E+02 4.48E+02 1.03E+03 4.94E+03 4.05E+01 4.98E+03
Module C1 0.00E+00 0.00E+00 0.00E+00 0.00E+00 0.00E+00 0.00E+00
Module C2 8.28E-01 0.00E+00 8.28E-01 5.34E+01 0.00E+00 5.34E+01
Module C3 6.01E+00 0.00E+00 6.01E+00 1.48E+02 0.00E+00 1.48E+02
Module C4 7.48E-01 0.00E+00 7.48E-01 7.70E+01 0.00E+00 7.70E+01
Module D -1.18E+01 0.00E+00 -1.18E+01 -3.68E+01 0.00E+00 -3.68E+01
LEGEND:
Product stage
End-of-life stage
Benefits and loads beyond the system boundary
EPR = use of renewable primary energy excluding renewable primary energy resources used as raw materials; RR = use of renewable primary energy resources
used as raw materials; TRR = total use of renewable primary energy resources (EPR + RR); EPNR = use of non-renewable primary energy excluding non-
renewable primary energy resources used as raw materials; RNR = use of non-renewable primary energy resources used as raw materials; TRNR = total use of
non-renewable primary energy resources (EPRN + RNR);
NOTE: Values expressed by declared unit (1 t of SECOLITE® boards).
Secondary materials and fuels, and use of water
MS CSR CSNR Net use of fresh water
Unit kg MJ, P.C.I. MJ, P.C.I. m3
Modules A1-A3 0.00E+00 0.00E+00 0.00E+00 8.17E+00
Module C1 0.00E+00 0.00E+00 0.00E+00 0.00E+00
Module C2 0.00E+00 0.00E+00 0.00E+00 1.41E-02
Module C3 0.00E+00 0.00E+00 0.00E+00 1.12E-01
Module C4 0.00E+00 0.00E+00 0.00E+00 1.04E-01
Module D 0.00E+00 0.00E+00 0.00E+00 -5.10E-01
LEGEND:
Product stage
End-of-life stage
Benefits and loads beyond the system boundary
MS = use of secondary material; CSR = use of renewable secondary fuels; CSNR = use of non-renewable secondary fuels.
NOTE: Values expressed by declared unit (1 t of SECOLITE® boards).
DAPHabitat System 12
2.5. Other environmental information describing different waste categories
Hazardous waste disposed Non-hazardous waste disposed Radioactive waste disposed
Unit kg kg kg
Modules A1-A3 9.69E-02 8.09E+01 8.97E-03
Module C1 0.00E+00 0.00E+00 0.00E+00
Module C2 3.40E-04 2.61E+00 1.73E-05
Module C3 8.27E-04 1.23E+02 1.80E-04
Module C4 4.46E-04 3.01E+02 1.29E-05
Module D -2.43E-04 -6.12E-01 -1.38E-04
LEGENDA:
Product stage
End-of-life stage
Benefits and loads beyond the system boundary
NOTE: Values expressed by declared unit (1 t of SECOLITE® boards).
The characteristics that make waste hazardous are described in the applicable legislation in force, for example in the European Waste Framework
Directive.
DAPHabitat System 13
2.6. Environmental information describing output flows
Components for re- Materials for Materials for energy
Exported energy
use recycling recovery
Unit kg kg kg MJ
Modules A1-A3 0.00E+00 1.04E+01 0.00E+00 0.00E+00
Module C1 0.00E+00 0.00E+00 0.00E+00 0.00E+00
Module C2 0.00E+00 0.00E+00 0.00E+00 0.00E+00
Module C3 0.00E+00 7.00E+02 0.00E+00 0.00E+00
Module C4 0.00E+00 0.00E+00 0.00E+00 0.00E+00
Module D 0.00E+00 0.00E+00 0.00E+00 0.00E+00
LEGEND:
Product stage
End-of-life stage
Benefits and loads beyond the system boundary
NOTE: Values expressed by declared unit (1 t of SECOLITE® boards).
The characteristics that make waste hazardous are described in the applicable legislation in force, for example in the European Waste Framework
Directive.
2.7. Information describing the biogenic carbon content at the factory gate
Biogenic carbon content* Units** Modules A1-A3 (results)
Biogenic carbon content in product kg C Not applicable (inorganic product)
Biogenic carbon content in accompanying packaging kg C 1.07E+01
* 1 kg biogenic carbon is equivalent to 44/12 kg of CO2.
** This information can be omitted whenever the content of biogenic carbon in the product, or in the respective packaging, is less than 5% of the
mass of the product, or the respective packaging.
3. SCENARIOS AND ADDITIONAL TECHNICAL INFORMATION
3.1. C1 De-construction, demolition – End of life of the product
It was assumed, as in the case of other types of finishing products, notably ceramic cladding waste by the EN
17160:2019 standard, that stage C1 is not relevant for cement cladding panels since the impacts resulting from this
stage are very small.
DAPHabitat System 14
3.2. C2 Transport – End of life of the product
The scenario considered at this stage is that recommended by the EN 17160:2019 standard, which corresponds to
transporting demolition waste from cement panels to a storage or treatment centre for construction or demolition
waste, using a lorry and considering an average transport distance of 20 km.
3.3. C3 Waste processing for reuse, recovery and/or recycling – End of life of the product
For modelling this stage, the scenario defined by the EN 17160:2019 standard was considered, where 70% of the
mass of the waste generated at the end of the product's useful life is processed so that it can be recycled.
3.4. C4 Disposal – End of life of the product
For the modelling of this stage, the scenario defined by the EN 17160:2019 standard was considered, which 30% of
the mass of waste generated at the end of the product's useful life is landfilled.
3.5. Scenario and technical information for module D
Results expressed per functional or declared unit
Parameter Units/comments
Scenario D
It was considered that 70% of the waste from SECOLITE® Cement Boards is
recovered for end-of-life valorization (conservative estimate) after
Scenario crushing and as a replacement for natural aggregates, according to
statistical data on Construction and Demolition Waste (CDW) from the
Portuguese Environment Agency (APA).
Net output flow specified per
Units as appropriate 700 kg per ton of SECOLITE® Cement Boards
material
Avoid production Units as appropriate 700 kg of natural aggregates per ton of SECOLITE® Cement Boards
Location of end-of-waste point At the recycling site
It is considered that the SECOLITE® board waste, after crushing, has a
Point of functional equivalence
quality similar to that of natural aggregates.
3.6. Additional information on release of dangerous substances to indoor air, soil, and
water during the use stage
This is irrelevant, as this product does not contain any potentially dangerous substances listed in Regulation (EC)
No 1907/2006 (REACH) in concentrations above 0.1%.
DAPHabitat System 15
4. REFERENCES
✓ General Instructions of the DAPHabitat System, Version 2.1, Edition August 2023 (in www.daphabitat.pt);
✓ PCR – basic module for construction products and services. DAPHabitat System. Version 2.3, August 2023 (in
www.daphabitat.pt);
✓ PCR - Wall covering. DAPHabitat System. Version 1.2, June 2022 (in www.daphabitat.pt);
✓ ISO 14025:2009 Environmental declarations and labels – Type III environmental declarations – Principles and
procedures;
✓ EN 15804:2012 + A2:2019 Sustainability of construction works – Environmental product declarations – Core
rules for the product category of construction products;
✓ EN 15942:2021 Sustainability of construction works – Environmental product declarations – Communication
format business-to-business.
✓ EN 17160:2019 Product category rules for ceramic tiles.
DAPHabitat System 16
