Logo of the EPD’s owner]
DAPHabitat System Environmental Product Declaration
www.daphabitat.pt [according to ISO 14025, EN 15804:2012+A2:2019 and EN 15942]
Declaration number: DAP 003:2023
PORTUGUESE “GREY” CEMENT
ISSUE DATE: 04/12/2023 VALID UNTIL: 03/12/2028
ATIC – ASSOCIAÇÃO TÉCNICA DA INDÚSTRIA DE CIMENTO
Version 1.4. Ed. September 2023
1
Index
1. GENERAL INFORMATION .................................................................................................................. 1
1.1. The DAPHAbitat System ............................................................................................................................... 1
1.2. EPD owner .................................................................................................................................................... 1
1.3. Information concerning the EPD .................................................................................................................. 2
1.4. Demonstration of the verification ............................................................................................................... 2
1.5. EPD Registration .......................................................................................................................................... 2
1.6. PCR (product category rules) basic model ................................................................................................... 3
1.7. Relevant c-PCR (Complementary product category rules) .......................................................................... 3
1.8. Information concerning the product/product class ..................................................................................... 4
1.9. Calculation rules of the LCA ......................................................................................................................... 6
1.10. Use of average environmental performance ............................................................................................... 7
1.11. Technical information for Reference Service Life (RSL) ............................................................................... 7
1.12. Flow diagram of input and output of the processes .................................................................................... 8
2. CORE ENVIRONMENTAL IMPACT INDICATORS ................................................................................ 9
2.1. Description of the system boundaries ......................................................................................................... 9
2.1.1. Justification for the exemption to declare modules C1, C2, C3, C4 and D ............................................ 10
2.2. Core environmental impact indicators ...................................................................................................... 11
2.3. Additional environmental impact indicators ............................................................................................. 11
2.4. Indicators describing resource use ............................................................................................................ 12
2.5. Other environmental information describing different waste categories ................................................. 12
2.6. Environmental information describing output flows ................................................................................. 12
2.7. Information describing the biogenic carbon content at the factory gate .................................................. 13
3. REFERENCES ................................................................................................................................... 14
DAPHabitat System
iii
1. GENERAL INFORMATION
1.1. The DAPHAbitat System
Associação Plataforma para a Construção
Sustentável
Program operator:
www.centrohabitat.net
centrohabitat@centrohabitat.net
Departamento Engenharia Civil
Address:
Universidade de Aveiro
3810-193 Aveiro
Email address: deptecnico@centrohabitat.net
Telephone number: (+351) 234 401576
www.daphabitat.pt
Website:
Logo
1.2. EPD owner
Name of the owner: ATIC – Associação Técnica da Indústria de Cimento
Praceta Teófilo Araújo Rato, 2600 - 540 ALHANDRA |
Rua dos Troviscais 10, 3020 - 886 SOUSELAS |
Cerro da Cabeça Alta - Apartado 45, 8100 - 952 LOULÉ |
Production site:
Estrada do Outão, 2900-718 SETÚBAL |
Maceira Liz-Maceira, 2405-018 LEIRIA |
Pataias-Gare – Apartado 46, 2449-909 PATAIAS |
Address (head office): Edifício Central Park, Rua Central Park, 6, 4ºC, 2795 - 242 LINDA-A-VELHA
Telephone: +351 213 510 830
E-mail: cimento.atic@atic.pt
Website: http://www.atic.pt/
Logo:
Information concerning the
applicable management Both producers are certified by the NP EN ISO 14001:2015 Environmental Management Systems
standard.
Systems:
Specific aspects regarding the
production: CAE 23510 – Cement Manufacture
Organization’s environmental
Not Applicable.
policy:
DAPHabitat System 1
1.3. Information concerning the EPD
Authors: c5Lab - Sustainable Construction Materials Association
Edifício Central Park, Rua Central Park 6 | 2795-242 LINDA-A-VELHA
Contact of the authors:
Email: fcapucha@c5lab.pt
Issue date:
04/12/2023
Registration date:
18/12/2023
Registration number:
DAP 003:2023
Valid until:
03/12/2028
Representativity of the EPD
(location, manufacturer, EPD for the average product “Grey” cement, manufactured in (6) six industrial plants from the (2) two
producers (Cimpor - Cimentos de Portugal, SGPS, S.A. | Secil - Companhia Geral De Cal E Cimento, S.A.).
group of manufacturers):
Where to consult explanatory
https://secilpro.com/
material: https://www.cimpor.com/cimento#produtos
Type of EPD: Cradle-to-Gate EPD (A1-A3)
1.4. Demonstration of the verification
External independent verification, accordingly, with the standard ISO 14025:2010 and EN 15804:2012+A2:2019
CERTIFICATION Body Verifier (s)
(CERTIF – Associação para a Certificação) (Ana Cláudia Dias, Marisa Almeida)
1.5. EPD Registration
Operador de Programa de Registo
(Plataforma para a Construção Sustentável)
DAPHabitat System 2
1.6. PCR (product category rules) basic model
Name: PCR: Basic module for construction products and services
Issue date: Edition August 2023
Number of registrations on the data
RCP-mb001
base:
Version: Version 2.3
Identification and contact of the Marisa Almeida | marisa@ctcv.pt
coordinator (s): Luís Arroja | arroja@ua.pt
José Dinis Silvestre | jose.silvestre@ist.utl.pt
Marisa Almeida | marisa@ctcv.pt
Identification and contact of the
Luís Arroja | arroja@ua.pt
authors: José Silvestre | jds@civil.ist.utl.pt
Fausto Freire
Cristina Rocha
Ana Paula Duarte
Ana Cláudia Dias
Helena Gervásio
Victor Ferreira
Ricardo Mateus
António Baio Dias
Composition of the Sectorial Panel: -
Consultation period: 18/11/2015 - 18/01/2016
Valid until: 01/06/2027
CEN standard EN 15804 serves as the core Product Category Rules (PCR)
1.7. Relevant c-PCR (Complementary product category rules)
Not Applicable.
DAPHabitat System 3
1.8. Information concerning the product/product class
Identification of the product: “Grey” Cement
Illustration of the product:
Brief description of the product: Cement is a hydraulic binder, i.e., a finely ground inorganic material which, when mixed
with water, forms a paste which sets and hardens by means of hydration reactions and
processes and which, after hardening, retains its strength and stability even under water.
The main raw materials (limestone and marl) are obtained from the internal quarries
localized in the plant’s premises. The corrective raw materials and additives (clay, shale,
sand, gypsum) are obtained from external quarries and transported to the plants. The
secondary raw materials come from waste produced by other sectors. The intermediary
product (clinker) is obtained in the rotary kiln which is localized in the plant’s premises.
Main technical characteristics of the The product class “grey” cement consists of a group of 12 products manufactured by the
product: two producers and listed in table 1.
Table 1: Composition of the product that make the class “grey” cement.
Blend/Producer EN 197-1 EN 197-1 Composition
Producer
Designation Designation requirements
95-100% Clinker
CEM I 52,5 R Portland Cement CIMPOR
0-5% Minor Additional Constituents
95-100% Clinker
CEM I 42,5 R Portland Cement CIMPOR
0-5% Minor Additional Constituents
80-94% Clinker;
Portland-Limestone
CEM II/A-L 42,5 R CIMPOR 6-20% Limestone (<0.5% TOC)
Cement
0-5% Minor Additional Constituents
65-79% Clinker
Portland-Limestone
CEM II/B-L 32,5 N CIMPOR 21-35% Limestone (<0.5% TOC)
Cement
0-5% Minor Additional Constituents
45-64% Clinker (3CaO.Al2O3<9%)
CEM IV/B (V) 32,5 N - Sulphate Resisting
CIMPOR 36-55% Fly Ash
SR Pozzolanic Cement
0-5% Minor Additional Constituents
65-79% Clinker (3CaO.Al2O3<9%)
CEM IV/A (V) 42,5 R – Sulphate Resisting
CIMPOR 36-55% Fly Ash
SR Pozzolanic Cement
0-5% Minor Additional Constituents
95-100% Clinker
CEM I 52,5 R Portland Cement SECIL
0-5% Minor Additional Constituents
95-100% Clinker
CEM I 42,5 R Portland Cement SECIL
0-5% Minor Additional Constituents
65-79% Clinker
Portland-Limestone
CEM II/B-L 42,5 R SECIL 21-35% Limestone (<0.5% TOC)
Cement
0-5% Minor Additional Constituents
65-79% Clinker
Portland-Limestone
CEM II/B-L 32,5 N SECIL 21-35% Limestone (<0.5% TOC)
Cement
0-5% Minor Additional Constituents
80-94% Clinker
Portland-Limestone
CEM II/A-L 42,5 R SECIL 6-20% Limestone (<0.5% TOC)
Cement
0-5% Minor Additional Constituents
65-79% Clinker (3CaO.Al2O3<9%)
CEM IV/A (V) 32,5 R – Sulphate Resisting
SECIL 36-55% Fly Ash
SR Pozzolanic Cement
0-5% Minor Additional Constituents
TOC – Total Organic Carbon
DAPHabitat System 4
Table 2 lists the products CE conformity declaration for each of the 12 products that
compose the “grey” cement class.
Table 2: CE conformity declarations for the products of the “grey” cement class.
Product Designation Producer CE Conformity Declaration
CEM I 52,5 R CIMPOR http://bit.ly/CEMI525R-CIMPOR
CEM I 42,5 R CIMPOR https://bit.ly/CEMI425R-CIMPOR
CEM II/A-L 42,5 R CIMPOR https://bit.ly/CEMIIA-L425R-CIMPOR
CEM II/B-L 32,5 N CIMPOR https://bit.ly/CEMIIB-L325N-CIMPOR
CEM IV/B (V) 32,5 N - SR CIMPOR https://bit.ly/CEMIVBV325N-SR-CIMPOR
CEM IV/A (V) 42,5 R – SR CIMPOR https://bit.ly/CEMIVAV425R–SR-CIMPOR
CEM I 52,5R SECIL https://bit.ly/CEMI525RSECIL
CEM I 42,5R SECIL https://bit.ly/CEMI425RSECIL
CEM II/B-L 42,5R SECIL https://bit.ly/CEMIIBL425RSECIL
CEM II/B-L 32,5N SECIL https://bit.ly/CEMIIB-L325NSECIL
CEM II/A-L 42,5R SECIL https://bit.ly/CEMIIA-L425RSECIL
CEM IV/A (V) 32,5R – SR SECIL https://bit.ly/CEMIVAV325-R-SR-SECIL
Description of the product’s Cement is used as a hydraulic binder that, when appropriately mixed with water and
application/use: aggregates, produces concrete, mortar or cement screed that retains its workability for a
sufficient time and, after a specified period, attains strength and long-term volume
stability.
Placing on the market / Rules of NP EN 197-1:2012 – Cement - Part 1: Composition, specifications, and conformity criteria
application in the market / Technical for common cements.
rules of the product: NP EN 14216:2015 – Cement - Composition, specifications, and conformity criteria for very
low heat special cements.
Quality control: Both producers are certified in the Quality Management Systems standard, EN ISO
9001:2015, thus assuring the manufacturing quality control within the industrial plants.
Special delivery conditions: Depending on the type of material and client necessities, “grey” cement can be delivered
in bulk, in kraft bags on top of wood pallets, on large, plasticized packages and big-bags.
Components and substances to declare:
Not Applicable.
Where explanatory material may be The information can be found at the following links:
https://www.secil.pt/pt/centro-de-documentacao
obtained:
https://www.cimpor.com/cimento#produtos
History of the LCA studies:
Not Applicable.
DAPHabitat System 5
1.9. Calculation rules of the LCA
Functional unit: Not Applicable.
Declared unit: 1 metric tonne of “grey” cement
System boundaries: Cradle-to-gate EDP. From the extraction and processing of raw materials until the product
enters into the dispatch procedure.
Criteria for the exclusion: The following unit processes complies with the exclusion criterion established on EN 15804,
corresponding to 1% of the total consumed energy or total input mass. The overall
neglected input flows per module must not be higher than 5% of the total energy or mass
input.
• Liquid Oxygen; • Griding Balls;
• Lixiviates; • Machinery Oils and Greases;
• Chromium VI Reducing Agents; • Acetylene;
• Baghouse Filters; • Refractories;
• Liquid CO2 Cylinder; • Sodium Hypochlorite;
• Biocides; • Descalers.
• Corrosion Protectors;
Assumption and limitations The primary data corresponds to the summation for the manufacture of 12 cement types
that compose the product class “Grey” cement, within the six industrial plants from the two
producers (CIMPOR and SECIL). Information was supplied consolidated and anonymised
therefore, it is not possible to disaggregate the inventory by type of cement or individual
industrial plant.
Quality and other characteristics about
The quality analysis was carried out based on the 'UN Environmental Global guidance on
the information used in the LCA: LCA database development' in accordance with the criteria stipulated in Annex E of EN
15804:2012+A2:2019. The quality of the data was categorised generically between
reasonable and very good on a 5-level qualitative scale from very poor to very good.
The information on the production of "grey" cement was obtained less than 5 years ago,
using mostly primary data collected directly from the industrial statistics of the six industrial
units and subsequently consolidated, being representative of the reality of production.
Information for background processes not provided by the industrial units, and over which
the producers have no influence, was obtained from generic data in the Ecoinvent 3.9.1
database (updated in June 2023), or by consulting the EPDs of equivalent products.
These were selected to provide geographical and technological coverage that fulfils the data
quality criteria stipulated in Annex E of EN 15804:2012+A2:2019. Electricity production was
modulated using information obtained directly from the regulator of energy production and
electricity infrastructure in Portugal. The results obtained are considered to be robust. The
LCA was carried out using SimaPro 9.5 software. Table 3 presents the composition of the
product modelled in SimaPro 9.5 (corresponding to the average composition of the
Portuguese “grey” cement):
Table 3 - Composition of the “grey” cement in the LCA model.
Constituents Amount kg (Per Declared Unit)
“Grey” Clinker 779
Gypsum 54
Filer 154
Own Limestone 7
Fly Ash 6
Total 1000
Allocation rules: Since the inventory data collected relates only to the production of "Grey" Cement, no
allocation procedure is deemed necessary. The polluter pays principle has been applied to
waste consumed in the process and waste produced that is subject to recovery processes.
Software used for the assessment: SimaPro 9.5 – PRé Sustainability
Background database used for the LCA: Ecoinvent Database v3.9.1 - Ecoinvent
Variability of LCIA results: The main factor affecting the variability of the LCIA results is the ratio of clinker consumed,
which can vary between 45% (for a CEM IV cement) and 97.5% (for CEM I). The average
clinker consumption rate is 77.9%. The percentages shown refer to the mass of the final
product. As clinker is a constituent with a significant environmental impact, mainly
associated with rotary kiln activity, the clinker content may affect the variability of the LCIA
results.
DAPHabitat System 6
Other parameters such as the clinker kilns fuel mix and additives used may also slightly
affect the LCIA results.
Comparability of EPD for construction The EPD of construction products and services cannot be comparable in case they are not
produced according to EN 15804 and EN 15948 and according to the comparability
products conditions determined by ISO 14025.
1.10. Use of average environmental performance
The present environmental declaration concerns a series of 12 products manufactured in six plants from two
producers (CIMPOR and SECIL) making the average product Portuguese “grey” cement. The technological
homogeneity between the manufacturing plants is high, the production method for each of the 12 products is
equivalent (Dry Process), only the ratio of constituent’s mixture, consumption of intermediary product and/or
additives, among other minor parameters varies. The main factor affecting the variability of the LCIA results is the
clinker content, which can vary between 45% (for a CEM IV cement) and 100% (for CEM I). The average clinker
consumption rate is 77.9 in weight percentage of the final product output.
While these factors may vary from cement plant to cement plant and cement blend to cement blend, the LCA
indicators for Portuguese “Grey” cement are within a range close enough to justify the application of the
representative EPD for its intended use, i.e., providing the basis for the environmental assessment of buildings and
other construction works in typical Portuguese situations. For detailed calculations requiring LCA data for specific
cements, please refer to individual cement companies.
1.11. Technical information for Reference Service Life (RSL)
Not applicable.
DAPHabitat System 7
1.12. Flow diagram of input and output of the processes
Raw Material Storage &
Quarrying Process Crusher Quarry
Preblending
Corrective and/or secondary materials
Limestone + Marl
Homogenising and Raw Meal Raw Mill Raw Milling
Storage of Raw Meal
Corrective and/or secondary materials
Clinker
Cyclone Pre-Heater Rotary Kiln Clinker Cooler
Sintering
Fossil and Alternative Fuels
Clinker
Cement Milling
Cement Storage Cement Cement Mill Clinker Storage
and Storage
Other main Gypsum
constituents
Figure 1: Flowchart for the cement manufacturing process.
System Boundaries – Manufacturing of Portuguese Grey Cement - 2018
• • A Sm O2m Ao bn sia o r– b e n 7 ts k –g 2 kg • W Maa ns ute fa f cro tum ri nC ge m – e n kt g T M2 4r . 6a R a1 .n ro 8 1is a t t tip d mk ko : m mert : • • • • • W I C S A Ca ro i l aas l uint l c mc +e a– i u ic Sn –m4o a i n 5 – k – –t . ga 8 4 4 2i .n k. . 95 8i gn k g k k ggg: T 2r .a R 6n o 4s a tp d ko : mrt • • • • P E F Gey l r. ir r tAi r t o –e r s c – i. t a S l a k– gg k –g k g kg G SS Cy Chap .l a anT M Ls l ydu ir e .Ra a m – ––r –n o i s a 6t 21 p i .d ..m 9 . 2 25o 2:. T e 9 r tt t kt k: k kt m mmk mm • • • • • S S C G Ca h l .ya Ln a py id l ms e – u – e– m . –k – g 2 k k 2g g 1 kk gg • • • D A LiNi me Fs ee O sl t, o –b n u e r n + e M d g arin rl M Exa t. . – – 9 9 7M kJ g
Internal Waste External Waste Subproducts External Quarries Internal Quarry
1 kg 21.9 kg 6.7 kg 304.1 kg 997 kg
(CCo linn ks eu rm Pa hb ale ss e) Secondary Raw Materials PoE rl te uc gt ari lc 2it 0y 18 Natural Raw Materials
0.9 kg 29.6 kg 88.5 kWh 1.30 t
• (T oF tao ls Tsi rl a F nu se pl os r - t: 6 30 5 2kg tkm) Combus Fti uo en l sof Fossil 1.7 GJ CR oo mta br uy sK tii oln n 2.9 GJ Production of 409 kg CO2 R D ae wc a Mrb ao ten ra iati lo sn of
Grey Clinker 7.5 gr
Clinker Phase• (T oA talt l. TF ru ae nls s p– o rt : 1 0 k 8g tkm) AC lto em rnb au tis vt eio Fn u o ef ls 1.2 GJ • • 2 33 .41 kk gg -- OC tO he2 r Polluents Em (i Css linio kn e ro f P P ha ar st eic )les
Cement Phase
Transport Transport
•
•
N Taa ptu Wra al O ter ri g –i n –
3 m
4 354 m3 GG yy Fpp ils esM uu rR m ma –or i –a–t .i d 22m : .0 t5e
k
t t mk km m • • • G F Oi wy lep nrs – Lu m i m e– . k – g k g kg 1 2R . .R1 8o a a t ti kk ld : mm: • Fly Ash – kg 779 kg • • M Oci cll uin pag t iA ond , j iu ndv ua sn trt ias l – ar e a – 1k .g 44E-4 ha
Water Consumption PoE rl te uc gt ari lc 2it 0y 18 Additives Alternative Additives Consumed Clinker PlaC no tn As ru em a a Ob cle cs u p& ie d
0.457m3 59 kWh 215 kg 6 kg 779 kg 0.3 kg
Em (Cis es mio en n o t f P P ha ar sti ec )les 5.1 gr
Production of Grey Cement
Waste Formation
Avoids 1 kg • HazardC ol uin s k Wer a sa tn ed S C ene tm toe n Dt i sP ph oa ss ae l s – gr 5.4 kg Grey Cement 1 t (1 tonne)
• Waste Sent to External Valorisation – 2.3 kg
• Waste Valorised Internally – .1 kg
Figure 2: Diagram depicting the overall inventory flows for producing one metric tonne of Portuguese “grey” cement.
DAPHabitat System 8
2. CORE ENVIRONMENTAL IMPACT INDICATORS
2.1. Description of the system boundaries
(✓= included; ND = module not declared)
BENEFITS AND LOADS
CONSTRUCTION
PRODUCT STAGE USE STAGE END OF LIFE STAGE BEYOND THE SYSTEM
PROCESS STAGE
BOUNDARY
y lp p u s la ire ta m w a R tro p s n a rT g n iru tc a fu n a M tro p s n a rT
s
s e c o r p n on io tcit ua rl tl sa nts n i e s U e c n a n e tn ia M ria p e R tn e m e c a lp e R tn e m h s ib ru fe R e s u y g re n e la n o ita re p O e s u re ta w la n o ita re p O n o itilo m e d ,s n o itc u rts n eo Dc
-
tro p s n a rT g n is s e c o rp e ts a W la s o p s iD g n ilc y c e r ,y re v o c e r ,e es Ru - la itn e to p
o
C
A1 A2 A3 A4 A5 B1 B2 B3 B4 B5 B6 B7 C1 C2 C3 C4 D
✓ ✓ ✓ ND ND ND ND ND ND ND ND ND ND ND ND ND ND
The system boundaries are limited to the Product Stage, covering the modules A1-A3. All “grey” cement
manufactured in the six plants is produced using the same method (Dry Process) described below:
Extraction and Processing of the Natural Raw Materials in the Quarry
Cement manufacturing starts in the internal quarry where the natural raw materials (limestone and marl) are
extracted. Localized in the factory premises, the quarry operates in open air through controlled explosions.
After extraction, the raw materials are presented in chunks with volumes up to 1 m3, being afterwards transported
by trucks to a crusher for granulometry reduction. Once at a reasonable granulometry, the raw material is stored
in pre-homogenising hangars.
Raw Meal Milling
In the manufacturing plant, the crushed natural raw materials are introduced in a mill (denoted ‘raw mill’) together
with secondary raw materials (e.g., pyrite) and corrective raw materials (e.g., sand), in predetermined dosages
according to the desired quality of the intermediary product (clinker), to produce the ‘Raw Meal’ a mixture with
very fine granulometries (lower than μm). Simultaneously, during milling, raw materials are dried using waste
heat from the rotary kiln hot gases exhaust. After milling, the raw meal is stored in silos. The secondary raw
materials and the corrective materials are transported to the factory gate from external quarries, raw materials
suppliers, or as waste from other sectors, mainly by road.
DAPHabitat System 9
Sintering
The raw meal is extracted from the silos and inserted in a cyclone system for pre-heating through the use of the
hot exhaust gases from the kiln. The pre-heated input will then enter the rotary kiln for sintering, slowly moving
across it by action of rotation and gravity. Inside the kiln, temperature reach up 1450 ºC promoting several
physicochemical reactions to obtain Clinker, an artificial rock with hydraulic properties. After sintering, the hot
clinker enters a cooling system which allows partial heat recovery by reintroducing the cooling air as secondary air.
The fossil and alternative fuels used in the rotary kiln are transported to the factory gate primarily via road or
maritime transport, being supplied from either fuel suppliers or as waste from other sectors.
Cement Milling and Storage
The final product, cement is produced by introducing mixture of clinker, gypsum, and other additives in a mill
(denoted ‘Cement Mill’). The ratio of mixture is carefully selected and scrutinised according to the desired
properties of the “grey” cement type that is intended to be produced, being stored in silos afterwards.
Dispatch
Cement can be commercialised in bulk, being directly extracted from the silos into cisterns. The dispatch process
and shipping to the construction stage (Module A4) is not covered by the system boundaries. The packaging
process is also excluded from the system boundaries.
2.1.1. Justification for the exemption to declare modules C1, C2, C3, C4 and D
“Grey” cement is an intermediary construction product that is physically integrated with other products (e.g.,
gravel, sand, and water) during construction phase, and goes through a chemical transformation (hydraulic
reactions) to create products such as concrete. It may have various end-uses, impossible to determine until its use
in the construction site, and it is not possible to separate it from the other products in the end-of-life. Moreover,
biogenic carbon is not present in the product, therefore according to EN 15804: 2012+A2: 2019, the product
system may be exempt from declaring the modules only the modules C1, C2, C3, C4 and D, declaring only the A1-
A3 modules, corresponding to the product stage.
DAPHabitat System 10
2.2. Core environmental impact indicators
Global warming Global warming Global warming Global warming Depletion Acidification
potential total; potential fossil; potential potential land potential of the potential;
biogenic; use and land use stratospheric
change; ozone layer;
GWP-total GWP-fossil GWP-biogenic GWP-luluc ODP AP
Unit kg CO2 eq. kg CO2 eq. kg CO2 eq. kg CO2 eq. kg CFC 11 eq. mol H+ eq.
Modules A1-A3 7.5E+02 7.3E+02 1.1E+01 8.2E-01 4.8E-06 6.6E-01
LEGEND:
Product Stage
Eutrophication Eutrophication Eutrophication Formation Abiotic depletion Abiotic depletion Water (user)
potential potential aquatic potential potential of potential for potential for deprivation
aquatic marine; terrestrial; tropospheric non-fossil fossil resources potential
freshwater; ozone; resources potential
ADP-
EP-freshwater EP-marine EP-terrestrial POCP ADP-fossil WDP
minerals&metals
Kg COVNM m3 world eq.
Unit kg P eq. kg N eq. mol N eq.
eq.
kg Sb eq. MJ, P.C.I
deprived
Modules A1-A3 1.7E-02 4.2E-01 1.7E+00 1.5E+00 2.4E-06 3.1E+03 6.0E+01
LEGEND:
Product Stage
Note: The results obtained for the indicators "Depletion Potential for Non-fossil Abiotic Resources (ADP- minerals&metals)", "Depletion Potential for Fossil Abiotic
Resources (ADP-fossil)" and "Water Unavailability Potential (user) (WDP)" should be used with caution as the uncertainties associated with them are high or there
is little experience with the indicator.
2.3. Additional environmental impact indicators
Potential Potential Human Potential Potential Potential Potential soil
incidence of exposure Comparative Comparative Comparative quality index
disease due to efficiency Toxic Unit for Toxic Unit for Toxic Unit for
PM emissions relative to U235 ecosystems humans, cancer humans, not
effects cancer effects
PM IRP ETP-fw HTP-c HTP-nc SQP
Disease
Unit kBq U 235 eq. CTUe CTUh CTUh -
incidence
Modules A1-A3 6.8E-06 3.1E+00 2.2E+03 1.1E-08 6.0E-07 8.8E+02
LEGEND:
Product Stage
Note: The impact indicator "Potential Human Exposure Efficiency in relation to U235 (IRP)" focuses mainly on the possible impact of a low dose of ionising
radiation on human health resulting from the nuclear fuel cycle. It does not consider effects arising from possible nuclear accidents, occupational exposure, or
the disposal of radioactive waste in underground facilities. Potential ionising radiation from soil, radon and some building materials is also not measured by this
indicator. The results obtained for the indicators "Comparative Toxic Potential Unit for Ecosystems (ETP-fw)", "Comparative Toxic Potential Unit for Humans,
Carcinogenic (HTP-c)", "Comparative Toxic Potential Unit for Humans, Non-Carcinogenic (HTP-nc)" and "Soil Quality Potential Index (SQP)" should be used with
caution as the uncertainties associated with them are high or there is little experience with the indicator.
DAPHabitat System 11
2.4. Indicators describing resource use
Primary Energy
EPR RR TRR EPNR RNR TRNR
Unit MJ, P.C.I. MJ, P.C.I. MJ, P.C.I. MJ, P.C.I. MJ, P.C.I. MJ, P.C.I.
Modules A1-A3 3.5E+02 0.0E+00 3.5E+02 3.1E+03 0.0E+00 3.1E+03
LEGEND:
Product Stage
EPR = use of renewable primary energy excluding renewable primary energy resources used as raw materials; RR = use of renewable primary energy resources
used as raw materials; TRR = total use of renewable primary energy resources (EPR + RR); EPNR = use of non-renewable primary energy excluding non-
renewable primary energy resources used as raw materials; RNR = use of non-renewable primary energy resources used as raw materials; TRNR = total use of
non-renewable primary energy resources (EPRN + RNR);
Secondary materials and fuels, and use of water
MS CSR CSNR Net use of fresh water
Unit kg MJ, P.C.I. MJ, P.C.I. m3
Modules A1-A3 3.6E+01 1.1E+02 1.1E+03 1.3E+00
LEGEND:
Product Stage
MS = use of secondary material; CSR = use of renewable secondary fuels; CSNR = use of non-renewable secondary fuels.
2.5. Other environmental information describing different waste categories
Hazardous waste disposed Non-hazardous waste disposed Radioactive waste disposed
Unit kg kg kg
Modules A1-A3 8.5E-02 4.0E-01 7.2E-04
LEGEND:
Product Stage
2.6. Environmental information describing output flows
Components for Materials for Materials for energy Exported energy
re-use recycling recovery
Energy carrier 1 … Energy carrier n
Unit kg kg kg MJ MJ MJ
Modules 6.9E-01 7.7E+00 1.4E-02 0.0E+00
LEGEND:
Product Stage
DAPHabitat System 12
2.7. Information describing the biogenic carbon content at the factory gate
Biogenic carbon content Units Modules A1-A3 (results)
Biogenic carbon content in product Kg C Not Applicable.
Biogenic carbon content in accompanying packaging Kg C Not Applicable.
DAPHabitat System 13
3. REFERENCES
✓ General Instructions of the DAPHabitat System, Version 2.1, Edition August 2023 (in www.daphabitat.pt );
✓ PCR – basic module for construction products and services. DAPHabitat System. Version 2.3, August 2023 (in
www.daphabitat.pt);
✓ ISO 14025:2009 Environmental declarations and labels – Type III environmental declarations – Principles and
procedures;
✓ EN 15804:2012 + A2:2019 Sustainability of construction works – Environmental product declarations – Core
rules for the product category of construction products;
✓ EN 15942:2021 Sustainability of construction works – Environmental product declarations – Communication
format business-to-business.
✓ ATIC - Associação Técnica da Indústria do Cimento, “Caracterização da Indústria,” 2 19.
✓ European Commitee For Standardization, EN 197-1:2 12 ‘Cement – Part 1: Composition, specifications, and
conformity criteria for common cements,’ 2 12th–04 ed. Brussels, 2011.
DAPHabitat System 14
