DAPHabitat System Environmental Product Declaration
[in accordance with ISO 14025, EN 15804:2012+A2:2019 and EN 15942]
www.daphabitat.pt
Registration number: EPD 014:2024
CEM I 52.5R PORTLAND CEMENT - OUTÃO
Issue date: 15/11/2024 Expiry date: 14/11/2029
SECIL - COMPANHIA GERAL DE CAL E CIMENTO, S.A.
Version 1.4.1 Ed. March 2024
Contents
1. GENERAL INFORMATION ................................................................................................................. 1
1.1. The DAPHabitat system .............................................................................................................................. 1
1.2. EPD Owner ................................................................................................................................................... 1
1.3. Information concerning the EPD ................................................................................................................. 2
1.4. Verification statement ................................................................................................................................ 2
1.5. Registration of the EPD ............................................................................................................................... 2
1.6. PCR (product category rules) basic model ................................................................................................. 3
1.7. c-PCR (complementary product category rules) ........................................................................................ 3
1.8. Product information/product class ............................................................................................................ 4
1.9. Calculation rules of the LCA ........................................................................................................................ 5
1.10. Use of average environmental performance ............................................................................................. 6
1.11. Technical information for Reference Service Life (RSL) ............................................................................. 6
1.12. Diagram of the process input and output flows ......................................................................................... 6
2. CORE ENVIRONMENTAL IMPACT INDICATORS............................................................................... 7
2.1. Description of the system boundaries ........................................................................................................ 7
2.1.1. Justification for the exemption to declare modules of C1, C2, C3, C4 and D ........................................... 8
2.2. Basic environmental impact indicators ...................................................................................................... 9
2.3. Additional environmental impact Indicators ........................................................................................... 10
2.4. Indicators describing the utilisation of resources .................................................................................... 11
2.5. Other environmental information describing different categories of waste .......................................... 11
2.6. Other environmental information describing output flows .................................................................... 12
2.7. Information describing the biogenic carbon content at the plant gate .................................................. 12
3. REFERENCES ................................................................................................................................... 13
DAPHabitat System
iii
1. GENERAL INFORMATION
1.1. The DAPHabitat System
Platform for Sustainable Construction Association
Identification of the programme www.clusterhabitat.pt
operator: geral@clusterhabitat.pt
University of Aveiro
Address: Department of Civil
Engineering
3810-193 Aveiro
Email address: deptecnico@clusterhabitat.pt
Telephone number: (+351) 234 401 576
Website: www.daphabitat.pt
Logo:
1.2. EPD Owner
Name of the owner: SECIL - Companhia Geral de Cal e Cimento, S.A.
Address (production site): Outão Plant
2901-864 Setúbal
Address (head office):
Estrada do Outão s/n,
2901-864 Setúbal
Telephone number: (+351) 217 927 100
Email address: apoiotecnico@secil.pt
Website: https://www.secil.pt/
Logo:
Information concerning NP EN ISO 9001 - Quality Management System NP
ISO 14001 - Environmental Management System
the applicable
ISO 45001 - Health and Safety Management System
management systems: and Health EMAS | Eco-Management Audit Scheme
Specific aspects regarding CAE (economic activity code) 23510 - Manufacture of cement
production:
Organization´s environmental
Commitments made by SECIL as part of its Environmental Responsibility and Protection
policy: policy:
• To ensure a responsible performance standard that makes using natural
resources compatible with the maintenance and development of the ecosystems
in which the company operates.
• To mitigate the impacts of its actions, through adopting the best technologies and
best practices available and the appropriate training of its employees.
• To promote biodiversity in the territories under its management. To reduce the
carbon impact of its activity, including by promoting the use of secondary raw
materials and alternative fuels.
To provide the public with regular data on its environmental performance.
DAPHabitat System
1
1.3. Information concerning the EPD
Authors:
Paula Quinteiro
Secil - Companhia Geral de Cal e Cimento, S.A.
Contact of the authors: Address: University of Aveiro, Santiago Campus, 3810-193 Aveiro, Portugal
Telephone: 234 370
200 E-mail:
p.sofia@ua.pt
Address: Estrada do Outão s/n, 2901-864 Setúbal, Portugal
E-mail: info.pssg@secil.pt
Issue date: 15/11/2024
Registration date: 22/11/2024
Registration number: EPD 014:2024
Valid until: 14/11/2029
Representativeness of the EPD of one (1) product class, produced in one (1) industrial unit, belonging to one (1) single
EPD (location, product, producer (Secil - Companhia Geral de Cal e Cimento, S.A)
group of
producers):
Where to find https://www.secil.pt/
product information:
Type of EPD Cradle-to-gate EPD (A1-A3)
1.4. Verification statement
Independent external verification in accordance with the NP ISO 14025:2010 and EN 15804:2012+A2:2019
standards
Certification Body Verifier(s)
(CERTIF – Associação para a Certificação) Marisa Almeida | José Dinis Silvestre
1.5. Registration of the EPD
Registration Programme Operator
(Platform for Sustainable Construction)
DAPHabitat System
2
1.6. PCR (product category rules) basic model
Name:
Base PCR model for construction products and services
Issue date:
Edition August 2023
Number of registration on the database:
RCP-mb001
Version:
Version 2.3
Identification and contact details of the Marisa Almeida | marisa@ctcv.pt
coordinator(s): Luís Arroja | arroja@ua.pt
José Dinis Silvestre | jose.silvestre@ist.utl.pt
Identification and contact of the authors: Marisa Almeida | marisa@ctcv.pt
Luís Arroja | arroja@ua.pt
José Silvestre | jds@civil.ist.utl.pt
Fausto Freire
Cristina Rocha
Ana Paula Duarte
Ana Cláudia Dias
Helena Gervásio
Victor Ferreira
Ricardo Mateus
António Baio Dias
Composition of the sector panel:
-
Consultation period:
18/11/2015 - 18/01/2016
Valid until:
01/06/2027
The CEN EN 15804 standard serves as the core product category rules (PCR).
1.7. c-PCR (complementary product category rules)
Name: EN 16908:2017+A1:2022 – Cement and building lime – Environmental product
declarations – Product category rules complementary to EN 15804
Issue date:
March 2022
Number of registration on the database:
EN 16908:2017+A1:2022
Version:
EN 16908:2017+A1, March 2022
Identification and contact of the
European Committee for Standardisation (CEN)
coordinator(s):
Identification and contact of the
-
authors:
Composition of the sector panel:
-
Consultation period:
-
Valid until:
-
DAPHabitat System
3
1.8. Product information/product class
Identification of the product: CEM I 52.5R Portland cement
Illustration of the product:
Brief description of the product: CEM I 52.5R Portland cement is a high-performance cement produced mainly from Portland
clinker - with an average composition of 95%-100% clinker and 0%-5% other components
under NP EN 197-1:2012. The clinker comes from Secil Outão.
The cement does not contain any substance included on the Candidate List of Substances of
Very High Concern (SVHC) above the limit for registration with the European Chemicals
Agency, i.e. above 0.1 per cent (m/m).
Main technical characteristics of the Table 1: Chemical, mechanical and physical characteristics of CEM I 52.5R Portland
product: cement.
Designation Units CEM I 52.5R Portland Standards
cement
Sulphate content (in SO3) % ≤ 4.0 NP EN 196-2
Chloride Content % ≤ 0.10 NP EN 196-2
First days:
2 days: ≥ 30
Compressive strength MPa NP EN 196-1
Reference: 28 days,
≥ 52.5
Start of setting min ≥ 45 NP EN 196-3
Expandability min ≤ 10.0 NP EN 196-3
Description of the application/use of CEM I 52.5R Portland cement is used in the manufacture of reinforced, prestressed or very
the high strength concrete and in situations where high strengths are required 1 or 2 days after
product: application.
CEM I 52.5R Portland cement is used in:
▪ ready-mixed or site-made concrete with high initial or final strength;
▪ pre-stressed concrete at very early ages;
▪ concrete applied in cold weather;
▪ heavy prefabrication with high mould turnover.
Placing on the market/Rules for CNP EN 197-1:2012 composition, specifications and conformity criteria for ordinary cements
application on the Conformity Certification
market/Technical
product standards:
Quality control: Not applicable
Special delivery conditions: Not applicable
Components and substances to Not applicable
declare:
Information where explanatory CEM I 52.5R Portland cement (nl) is available for sale to the general public
documents can be For detailed information about the product, please contact SECIL by e-mail
info.pssg@secil.pt
obtained:
History of LCA studies: --
DAPHabitat System
4
1.9. Calculation rules of the LCA
Functional unit: Not applicable
Declared unit: 1 000 kg of CEM I 52.5R Portland cement
System boundaries: The system evaluated includes the A1-A3 module (product stage). A more detailed
description of the system boundary is given in Section 2.1.
Criteria for the exclusion: The LCA considered the extraction and processing of natural raw materials, the production
of auxiliary materials and the energy consumed in the manufacture of CEM I 52.5R Portland
cement. As the Portland clinker produced at Secil is the main raw material, the extraction
and processing of natural raw materials and the transport of secondary raw materials
(waste from other industries) were also considered. The waste management processes
generated in the production of clinker (until the end of waste status is reached) for which
inventory data is available were considered.
CEM I 52.5R Portland cement also excluded grinding bodies, bag filters, lubricating oils and
the production of acetylene used in maintenance operations (welding). In clinker, bag filters,
the refractory lining of the kiln, lubricating oils, the production of acetylene used in
maintenance operations (welding), sodium hypochlorite, sodium hydroxide, chlorine and
the biocide used for water treatment were excluded from the system boundary, as they
correspond to a mass of less than 1% of the total mass of inputs. The total mass of input
from the unit processes does not exceed 5% of the total mass of inputs and is therefore
covered by the exclusion criterion defined in document EN 16908:2017+A1 - Cement and
building lime - Environmental product declarations - Product category rules, namely its mass
is less than 1% of the total mass of inputs.
In the LCA for Portland cement, it should be noted that the energy and water consumption
of the administrative areas, as well as the production of wastewater and waste from these
areas, were not included. In addition, environmental loads associated with the construction
and maintenance of infrastructure and equipment (capital goods) were excluded.
Assumptions and limitations: The results of the environmental impacts and other indicators presented in this EPD refer to
the year 2022.
Quality and other characteristics The quality of the inventory data was assessed taking into account the criteria of the PEF
of the information used in the LCA: (Product Environmental Footprint) category rules (section 5.6 of the guide, Menfredi et al.,
2012), as indicated in table E.2 (Data quality and criteria from the Product Environmental
Footprint Category Rules) of EN 15804:2012+A2:2019+AC and in the guide to the software
used, the GCCA EPD Tool for Cement and Concrete (V 4.2), and based on the
recommendations of the PCR documents - Base Model. The data quality was broadly
classified between reasonable and good on a 5-level qualitative scale from very bad to very
good, in line with the data quality requirements - temporal, geographical and technological.
The information on the production of CEM I 52.5R Portland cement is less than 5 years old,
using mostly primary data collected directly from SECIL - Outão Plant.
Real and specific data from the production unit was used for the operations associated with
the process of manufacturing CEM I 42.5R Portland cement. The information for background
processes not provided by SECIL, and over which SECIL has no influence, was obtained from
generic data in the Ecoinvent database v3.5. These were selected to provide geographical
and technological coverage that fulfils the data quality criteria stipulated in Annex E of EN
15804:2012+A2:2019.
Electricity production was modelled in the GCCA with information on the mix of energy
sources from the International Energy Agency (IEA).
Allocation rules: To determine the inputs and outputs associated only with the production of CEM I 52,5R
Portland cement, the procedure for subdividing the unit process was first adopted, following
the recommendations of the PCR document - Base Model. Thus, only the operations
associated with the production of the product being analysed were considered, and
operations exclusive to other products were excluded. Then, an allocation procedure was
applied for the operations included based on the mass of the different products produced.
Software used for the assessment: GCCA EPD Tool for Cement and Concrete (V 4.2), International version.
Background database used Ecoinvent database version 3.5 published in December 2018; cut-off approach.
for the LCA:
Variability of the results of LCIA The main factor affecting the variability of LCIA results will be the clinker content used in the
production of CEM I 52.5R Portland cement, which can vary from 87.5% to 94.0%, with the
average clinker consumption being 91%. This variability in cement composition resulted in a
variability of less than 5 per cent in the LCIA results.
Comparability of EPD construction EPD for construction products and services may not be comparable if they are not produced
products' : under EN 15804 and EN 15942 and the comparability conditions determined by ISO 14025.
DAPHabitat System
5
1.10. Use of average environmental performance
Not applicable
1.11. Technical information for Reference Service Life (RSL)
Not applicable
1.12. Diagram of the process input and output flows
Figure 1: Flowchart of the manufacturing process of CEM I 52.5R Portland cement
DAPHabitat System
6
2. CORE ENVIRONMENTAL IMPACT INDICATORS
2.1. Description of the system boundaries
(✓= included; ND = module not declared)
PRODUCT CONSTRUCTION USE STAGE END OF LIFE STAGE ENVIRONMENTAL
STAGE PROCESS STAGE BENEFITS AND
BURDENS BEYOND
THE SYSTEM
BOUNDARY
n o g n
s
la i r e t a m w Ra t r o p s n a r T g n ir u t c a f u n a M t r o p s n a r T
d n a
n o it c u r ts n o C
s s e c o
r p n o it a lla ts n i e s U e c n a n e t n i a M g n ir ia p e R t n e m e c a l p e R n o it a r o ts e R
e s u
y g r e n e la n o it a r e p
O
e s u
r e t a w la n o it a r e p O
itilo
m e d
d n a n o it c u r ts n o c e
D
t r o p s n a r T g n is s e c o r p e ts a W la s o p s iD
ilc
y c e r la
itn e t o p ,y r e v o c e r
,e
s
u
e
R
A1 A2 A3 A4 A5 B1 B2 B3 B4 B5 B6 B7 C1 C2 C3 C4 D
✓ ✓ ✓ ND ND ND ND ND ND ND ND ND ND ND ND ND ND
Module A1-A3 (product stage) of CEM I 52.5R Portland cement considers the extraction and processing of primary (natural) raw materials, the
production of auxiliary materials, the transport of raw materials, fuels and electricity to the production unit, Secil Outão.
The production of CEM I 52.5R Portland cement requires Portland clinker, gypsum and ground limestone as the main raw materials. The clinker
is produced at Secil Outão. The limestone comes from the Outão quarry. Mining is carried out above ground, on plateaus, starting at the highest
level. In line with good environmental practice, the quarry's paths are watered to minimise the effect of dust during the exploration phase and
the landscape recovery of the floors that have already been explored is guaranteed, under the approved Environmental and Landscape
Recovery Plan. The plaster comes from external production.
The main raw materials used to produce Secil Portland clinker are marl or clay and limestone. Once the materials are extracted from the quarry,
they are in the form of blocks measuring up to 1m3, so it is necessary to reduce their size to a dimension compatible with the transportation,
storage and supply of the subsequent manufacturing phases; this operation is performed in the crusher. After crushing, the natural raw
materials are transported by conveyor belt for storage. The limestone is stored in vertical silos, while the marl and secondary raw materials are
stored in a horizontal, circular hangar that allows for the pre-homogenisation of these materials.
This is followed by raw milling, in which the natural and secondary raw materials (materials derived from waste, e.g. concrete sludge,
calcination waste, lime sludge, kiln linings, construction and demolition waste) are subjected to a drying, milling and homogenising process.
Once the proportion of raw materials has been defined, they are transported to mills where the "flour" or “raw” material is produced, i.e. a
finely ground mixture, in well-defined proportions, of all the natural and secondary raw materials. The mill works by injecting water to stabilise
the grinding track layer. The water will mix with the raw materials creating a layer height necessary for the grinding process to be efficient. The
hot gases coming from the kiln will feed the mill, which will cause some of the water to evaporate, making it necessary to replace it (make-up).
This make-up therefore corresponds to actual water consumption. This water comes from the company's boreholes and requires treatment
with sodium hypochlorite, sodium chloride, bio-dispersant, chlorine and disinfectant to eliminate bacteria and prevent calcification in the
equipment. During milling, the "raw" material is also dried, using the heat contained in the exhaust gases of the rotary kiln.
This is followed by the preheating stage in which the raw material is extracted from the storage silos and fed into the preheating system
(cyclone tower), where it is heated by the exhaust gases resulting from the burning of the fuels in the rotary kiln. The raw material then goes
into the kiln and moves along it by rotation and a slight inclination, with heating continuing and the physio-
DAPHabitat System
7
chemical reactions at a temperature of up to 1450ºC to ultimately produce clinker. As firing is an energy-intensive stage, primary fuels are used,
i.e. fossil fuels, as well as secondary fuels (fuels derived from waste, e.g. used tyres, fluff - the non-recyclable textile component of tyres and
refuse-derived fuels (RDF)).
From 1450ºC onwards, the clinker begins to cool, still inside the kiln, and is completed in the cooler, where counter-current air is introduced,
using this heated air as secondary and tertiary firing air. This air is generated by the cooler's fans and is then divided into secondary air, which
goes into the kiln, and tertiary air, which is the air needed for combustion in the calciner. In this way, there is a partial recovery of the clinker's
thermal content to reduce energy consumption in the kilns. Particle matter emissions are controlled by dedusting systems and gas emissions
into the air by automated control systems for driving the kilns. The clinker is stored and then used to produce CEM I 52.5R Portland cement.
The transport of clinker to the mills is carried out with bag filters to minimise diffuse dust emissions. The cement is produced in horizontal
tubular mills. Clinker, gypsum (cement setting regulator), limestone and grinding aids, in well-defined proportions, according to the quality plan,
to obtain CEM I 52.5R Portland cement, which is stored in silos. The cement is ground in a closed circuit using 3rd generation separators. Also,
to minimise diffuse dust emissions, the cement mill has bag filters. Spot monitoring of total suspended particulate emissions is carried out.
CEM I 52.5R Portland cement is sold in bulk.
During clinker production, the diesel used for internal movements at the Secil plant and quarry comes from diesel refuelling stations at the
plant and quarry. Therefore, pollutant emissions to rainwater from hydrocarbon separators associated with the diesel refuelling station and the
collection of oily water throughout the plant and in the quarry, associated with the workshop and diesel refuelling station, were considered.
The diesel consumption of emergency generators was also considered to guarantee the normal operation of clinker production processes in the
event of a temporary power cut. The transport and treatment of waste resulting from the clinker production process, such as waste containing
hydrocarbons, was considered.
During Portland cement production, the diesel used for internal movements at the Secil plant and quarry comes from diesel refuelling stations
at the plant and quarry. Pollutant emissions to rainwater from the hydrocarbon separators associated with the diesel refuelling station and the
collection of oily water throughout the plant and on the wharf were therefore considered.
The production of CEM I 52.5R Portland cement and its subsequent sale in bulk does not result in the generation of waste.
2.1.1. Justification for the exemption to declare modules C1, C2, C3, C4 and D
CEM I 52.5R Portland cement, being an intermediate product, fulfils all the conditions required by EN 15804:2012+A2:2019+AC and EN 16908:2017
+A1, to consider the cradle-to-gate life cycle (A1-A3), namely:
▪ cement is a raw material with a wide range of potential applications, and it is not possible a priori to establish a single reference service
life;
▪ cement is physically integrated with other products, such as aggregates, into downstream products, such as concrete, mortar, etc., so it
is not possible to physically separate it at the end of its life;
▪ the cement is not identifiable at the end of its life as the result of a physical or chemical transformation process
▪ cement does not contain biogenic carbon and is exempt from the obligation to declare modules C1-C4 and D.
DAPHabitat System
8
2.2. Basic environmental impact indicators
Global Global Global warming
Global Depletion
warming warming potential - Land
warming potential of the Acidification
potential potential - use and land
potential - stratospheric potential;
total; fossil fuels; use change;
biogenic; ozone-layer;
AP
GWP-total GWP-fossil GWP-luluc
GWP-biogenic ODP
Unit kg CO2 eq. kg CO2 eq. kg CO2 eq. kg CO2 eq. kg CFC 11 eq. mol H+ eq.
Module A1-A3 8.07E+02 8.07E+02 2.59E-02 8.59E-02 1.71E-05 1.35E+00
LEGEND:
Product Stage
Units expressed per declared unit (1000 kg CEM I 52.5R Portland cement).
Eutrophicati Terrestrial Abiotic Abiotic
Eutrophication Formation Water (user)
on potential eutrophication depletion depletion
potential of potential deprivation
of aquatic potential; potential for potential
aquatic tropospheric potential;
freshwater; non-fossil for fossil
marine; ozone
resources; resources;
EP-
formation; WDP
EP-marine EP-terrestrial
freshwater ADP- ADP-fossil
POCP
minerals &
metals
m3 eq. of water
Unit kg P eq. kg N eq. mol N eq. Kg COVNM eq. kg Sb eq. MJ, P.C.I globally
unavailable
Module A1-A3 9.65E-03 9.94E-04 4.93E+00 1.33E+00 1.61E-04 3.30E+03 3.50E+01
LEGEND:
Product Stage
Units expressed per declared unit (1000 kg CEM I 52.5R Portland cement).
The results obtained for the indicators “Abiotic depletion potential for non-fossil resources (ADP-minerals&metals)”, “Abiotic depletion potential for fossil resources
potential (ADP-fossil)” and “Water (user) deprivation potential (WDP)” should be used with caution since the uncertainties associated with them are high or there is
little experience with the indicator
DAPHabitat System
9
2.3. Additional environmental impact indicators
Potential Potential Potential
Potential Potential Potential soil
human Comparative Comparative
incidence of Comparative quality index
exposure Human Toxicity Human Toxicity
disease due to Toxic Unit for
efficiency in Unit, carcinogenic Unit, non-
emissions of fine ecosystems SQP
relation to carcinogenic
particulate matter
U235 HTP-c
PM ETP-fw
HTP-nc
IRP
Incidence
Unit kBq U 235 eq. CTUe CTUh CTUh -
of disease
Module A1-A3 1.68E-05 4.87E+00 6.17E+01 1.28E-06 1.74E-05 2.21E+03
LEGEND:
Product Stage
Units expressed per declared unit (1000 kg CEM I 52.5R Portland cement).
The impact indicator “potential human exposure efficiency relative to U235” focuses mainly on the possible impact of a low dose of ionising radiation on
human health resulting from the nuclear fuel cycle. It does not consider effects arising from possible nuclear accidents, occupational exposure or the disposal
of radioactive waste in underground facilities. Potential ionising radiation from soil, radon and some building materials is also not measured by this indicator.
The results of the indicators “potential comparative toxic unit for ecosystems (ETP-fw)”, “potential comparative toxic unit for humans, cancer effects”, “potential
comparative toxic unit for humans, not cancer effects” and “potential soil quality index” should be used with caution as the uncertainties associated with them
are high or there is little experience with the indicator.
DAPHabitat System
10
2.4. Indicators describing the utilisation of resources
Primary energy
EPR RR TRR EPNR RNR TRNR
Unit MJ, P.C.I MJ, P.C.I MJ, P.C.I MJ, P.C.I MJ, P.C.I MJ, P.C.I
Module A1-A3 1.64E+03 0.00E+00 1.64E+03 3.30E+03 0.00E+00 3.30E+03
LEGEND:
Product Stage
Units expressed per declared unit (1000 kg CEM I 52.5R Portland cement).
EPR = use of renewable primary energy excluding renewable primary energy resources used as raw materials; RR = use of renewable primary energy resources
used as raw materials; TRR = total use of renewable primary energy resources (EPR + RR); EPNR = use of non-renewable primary energy excluding non-renewable
primary energy resources used as raw materials; RNR = use of non-renewable primary energy resources used as raw materials; TRNR = total use of non-
renewable primary energy resources (EPRN + RNR).
Secondary material and fuel, and water use
Net value of fresh
SM RSF NRSF
water
Unit kg MJ, P.C.I MJ, P.C.I m3
Module A1-A3 7.53E+01 2.89E+02 7.75E+02 8.73E-01
LEGEND:
Product Stage
Units expressed per declared unit (1000 kg CEM I 52.5R Portland cement).
SM = use of secondary material; RSF= use of renewable secondary fuels; NRSF = use of non-renewable secondary fuels; Fresh water = use of the net value of fresh
water.
2.5. Other environmental information describing different categories of waste
Non-hazardous waste
Hazardous waste disposed Radioactive waste disposed
disposed
Unit kg kg kg
Modul A1-A3 1.92E-01 1.30E-03 0.00+00
LEGEND:
Product Stage
Units expressed per declared unit (1000 kg CEM I 52.5R Portland cement).
The characteristics that make waste hazardous are described in the applicable legislation in force, for example in the European Waste Framework Directive.
DAPHabitat System
11
2.6. Other environmental information describing output flows
Components Materials Materials for Exported energy
for reuse for energy
recycling recovery
Unit kg kg kg MJ
Module A1-A3 0.00E+00 1.88E+00 8.40E+00 0.00E+00
LEGEND:
Product Stage
Units expressed per declared unit (1000 kg CEM I 52.5R Portland cement).
The characteristics that make waste hazardous are described in the applicable legislation in force, for example in the European Waste Framework Directive.
2.7. Information describing the biogenic carbon content at the plant gate
Biogenic carbon content* Units** Module A1-A3 (results)
Biogenic carbon content in the product Kg C Not applicable
Biogenic carbon content in accompanying packaging Kg C Not applicable
* 1 kg of biogenic carbon is equivalent to 44/12 kg of CO2
**
DAPHabitat System
12
3. REFERENCES
✓ GCCA (2023). GCCA Industry EPD Tool for cement and concrete (V4.0). Global Cement and Concrete Association
(GCCA) Quantis, Switzerland;
✓ DAPHabitat System General Instructions, Version 2.1, August 2023 (at www.daphabitat.pt);
✓ PCR - Base Model. Construction products and services. In accordance with EN 15804:2012+A2:2019.
DAPHabitat System. Version 2.3, August 2023 (at www.daphabitat.pt);
✓ NP ISO 14025:2009 Environmental labelling and declarations - Type III environmental declarations - Principles
and procedures;
✓ EN 15804:2012+A2:2019+AC Sustainability of construction works - Environmental product declarations - Core
rules for the product category of construction products;
✓ EN 16908:2017+A1 - Cement and building lime - Environmental product declarations - Product category rules
complementary to EN 15804 European Committee for Standardisation;
✓ EN 15942:2021 Sustainability of construction works – Environmental product declarations – Communication
format business-to-business;
✓ IEA (2024). Portugal - Countries & Regions. International Energy Agency (IEA).
https://www.iea.org/countries/portugal/electricity, accessed June 2024.
✓ Manfredi S., Allacker K., Chomkhamsri K., Pelletier N., Maia de Souza D. (2012). Product Environmental
Footprint (PEF) Guide. European Commission (EC), Joint Research Centre (JRC), Ispra, Italy;
✓ Secil (2023). Secil CO2 Manual. Monitoring, calculating and reporting CO2 emissions. Period 2021-2025. Version
06.
DAPHabitat System
13
