Applicant's logo]
DAPHabitat System Environmental Product Declaration
www.daphabitat.pt [in accordance with ISO 14025, EN 15804:2012+A2:2019 and EN 15942]
Registration number: EPD 013:2024
OUTÃO PORTLAND CLINKER
Issue date: 15/11/2024 Expiry date: 14/11/2029
SECIL - COMPANHIA GERAL DE CAL E CIMENTO, S.A.
Version 1.4.1 Ed. March 2024
Contents
1. GENERAL INFORMATION ................................................................................................................. 1
1.1. The DAPHabitat system .............................................................................................................................. 1
1.2. EPD Owner ................................................................................................................................................... 1
1.3. Information concerning the EPD ................................................................................................................. 2
1.4. Verification statement ................................................................................................................................ 2
1.5. Registration of the EPD ............................................................................................................................... 2
1.6. PCR (product category rules) basic model .................................................................................................. 3
1.7. c-PCR (complementary product category rules) ........................................................................................ 3
1.8. Product information/product class ............................................................................................................ 4
1.9. Calculation rules for LCA ............................................................................................................................. 5
1.10. Use of average environmental performance ............................................................................................. 6
1.11. Technical information for Reference Service Life (RSL) ............................................................................. 6
1.12. Diagram of the process input and output flows ......................................................................................... 6
2. CORE ENVIRONMENTAL IMPACT INDICATORS............................................................................... 7
2.1. Description of the system boundaries ........................................................................................................ 7
2.1.1. Justification for the exemption to declare modeules of C1, C2, C3, C4 and D .......................................... 8
2.2. Basic environmental impact indicators ...................................................................................................... 9
2.3. Additional environmental impact indicators ........................................................................................... 10
2.4. Indicators describing the utilisation of resources .................................................................................... 11
2.5. Other environmental information describing different categories of waste .......................................... 11
2.6. Other environmental information describing output flows .................................................................... 12
2.7. Information describing the biogenic carbon content at the plant gate .................................................. 12
3. REFERENCES ................................................................................................................................... 13
DAPHabitat System
iii
1. GENERAL INFORMATION
1.1. DAPHabitat registration system
Platform for Sustainable Construction Association
Identification of the programme
www.clusterhabitat.pt
operator:
geral@clusterhabitat.pt
University of Aveiro
Address: Department of Civil
Engineering
3810-193 Aveiro
Email address: deptecnico@clusterhabitat.pt
Telephone number: (+351) 234 401 576
Website: www.daphabitat.pt
Logo:
1.2. EPD Owner
Name of the owner: SECIL - Companhia Geral de Cal e Cimento, S.A.
Address (production site):
Outão Plant
2901-864 Setúbal
Address (head office):
Estrada do Outão s/n,
2901-864 Setúbal
Telephone number: (+351) 217 927 100
Email address: apoiotecnico@secil.pt
Website: https://www.secil.pt/
Logo:
Information concerning the NP EN ISO 9001 - Quality Management System NP
ISO 14001 - Environmental Management System
applicable management
ISO 45001 - Health and Safety Management System
systems:
and Health EMAS | Eco-Management Audit Scheme
Specific aspects regarding CAE (economic activity code) 23510 - Manufacture of cement
production:
Organization´s environmental
Commitments made by SECIL as part of its Environmental Responsibility and Protection
policy: policy:
• To ensure a responsible performance standard that makes the use of natural
resources compatible with the maintenance and development of the ecosystems
in which the company operates.
• To mitigate the impacts of its actions, through the adoption of the best
technologies and best practices available and the appropriate training of its
employees.
• To promote biodiversity in the territories under its management. To reduce the
carbon impact of its activity, including by promoting the use of secondary raw
materials and alternative fuels.
To provide the public with regular data on its environmental performance.
DAPHabitat System
1
1.3. Information concerning the EPD
Authors:
Paula Quinteiro
Secil - Companhia Geral de Cal e Cimento, S.A.
Contact of the authors: Address: University of Aveiro, Santiago Campus, 3810-193 Aveiro, Portugal
Telephone: 234 370
200 E-mail:
p.sofia@ua.pt
Address: Estrada do Outão s/n, 2901-864 Setúbal, Portugal
E-mail: info.pssg@secil.pt
Issue date: 15/11/2024
Registration date: 22/11/2024
Registration number: EPD 013:2024
Valid until: 14/11/2029
Representativeness of the EPD of one (1) product class, produced in one (1) industrial unit, belonging to one (1) single
EPD (location, product, producer (Secil - Companhia Geral de Cal e Cimento, S.A)
group of
producers):
Where to find https://www.secil.pt/
product information:
Type of EPD Cradle-to-gate EPD (A1-A3)
1.4. Verification Statement
Independent external verification in accordance with the NP ISO 14025:2010 and EN 15804:2012+A2:2019
standards
Certification Body Verifier(s)
(CERTIF – Associação para a Certificação) (Marisa Almeida | José Dinis Silvestre)
1.5. Registration of the EPD
Registration Programme Operator
(Platform for Sustainable Construction)
DAPHabitat System
2
1.6. PCR (product category rules) basic model
Name:
Base PCR model for construction products and services
Issue date:
Edition August 2023
Database registration number:
RCP-mb001
Version:
Version 2.3
Identification and contact details of the Marisa Almeida | marisa@ctcv.pt
coordinator(s): Luís Arroja | arroja@ua.pt
José Dinis Silvestre | jose.silvestre@ist.utl.pt
Identification and contact of the authors: Marisa Almeida | marisa@ctcv.pt
Luís Arroja | arroja@ua.pt
José Silvestre | jds@civil.ist.utl.pt
Fausto Freire
Cristina Rocha
Ana Paula Duarte
Ana Cláudia Dias
Helena Gervásio
Victor Ferreira
Ricardo Mateus
António Baio Dias
Composition of the sector panel:
-
Consultation period:
18/11/2015 - 18/01/2016
Valid until:
01/06/2027
The CEN EN 15804 standard serves as the basic product category rules (PCR).
1.7. c-PCR (complementary product category rules)
Name: EN 16908:2017+A1:2022 – Cement and building lime – Environmental product
declarations – Product category rules complementary to EN 15804
Issue date:
March 2022
Number of registration on the database:
EN 16908:2017+A1:2022
Version:
EN 16908:2017+A1, March 2022
Identification and contact of the
European Committee for Standardisation (CEN)
coordinator(s):
Identification and contact of the
-
authors:
Composition of the sector panel:
-
Consultation period:
-
Valid until:
-
DAPHabitat System
3
1.8. Product information/product class
Identification of the product: Clinker for Portland cement or Portland clinker for short.
Product illustration:
Brief description of the product: The main raw materials used to produce Portland clinker are marl and limestone, which are
extracted in quarries. Mining is carried out above ground, on plateaus, starting at the
highest level. In line with good environmental practice, the quarry's paths are watered to
minimise the effect of dust during the exploration phase and the landscape recovery of the
floors that have already been explored is guaranteed, under the approved Environmental
and Landscape Recovery Plan.
The natural raw materials and secondary materials (e.g. correction materials) are ground,
dosed and subjected to firing in which the physical-chemical reactions (calcination) of the
clinker process take place, to obtain Portland clinker. Portland clinker is a fine granular
material used as a binder in cement.
The clinker does not contain any substance included on the Candidate List of Substances of
Very High Concern (SVHC) above the limit for registration with the European Chemicals
Agency, i.e. above 0.1 per cent (m/m).
Main technical characteristics of the
Table 1: Technical characteristics and physical properties of Portland clinker.
product:
Designation Units Portland Clinker
Density g/cm3 Apparent 0.90 to 1.80
Solubility in water (T - 200C) g/l Mild (0.1 - 1.5)
pH (T = 200C; in water, water-solid ratio 1:2) - 11.0 - 13.5
Melting point ºC Greater than 1250
Odour; Odour threshold - Odourless; No threshold
Description of the application/use of For the production of Portland cements and other hydraulic binders
the
product:
Placing on the market/Rules for CNP EN 197-1:2012 composition, specifications and conformity criteria for ordinary cements
application on the
market/Technical
product standards:
Quality control: Not applicable
Special delivery conditions: Not applicable
Components and substances to Not applicable
declare:
Information where explanatory Portland clinker is an intermediate material for physical integration into cement that is not
documents can be available for sale to the general public.
obtained: For detailed information on the product, please contact SECIL at
info.pssg@secil.pt.
History of LCA studies: --
DAPHabitat System
4
1.9. Calculation rules of the LCA
Functional unit: Not applicable
Declared unit: 1,000 kg of Portland clinker
System boundaries: The system evaluated includes the A1-A3 module (product stage). A more detailed
description of the system boundary is given in Section 2.1.
Criteria for the exclusion: The LCA considered the extraction and processing of natural raw materials, the transport of
secondary raw materials (waste from other industries), the production of auxiliary materials
and the energy consumed in the manufacture of clinker. Likewise, the waste management
processes generated in clinker production (until the end of waste status is reached) for
which inventory data is available were considered. Excluded from the system boundary are
bag filters, kiln refractory lining, lubricating oils, the production of acetylene used in
maintenance operations (welding), sodium hypochlorite, sodium hydroxide, chlorine and
biocide used for water treatment, which individually corresponds to a mass of less than 1%
of the total mass of inputs, and as a whole correspond to a mass of less than 5% of the total
mass of inputs for each module. They are therefore covered by the exclusion criteria defined
in EN 16908:2017+A1 - Cement and building lime - Environmental product declarations -
Product category rules, namely their mass is less than 1% of the total mass of the inputs and
does not exceed 5% of the total mass of the inputs of each module. The LCA for Portland
clinker also excluded energy and water consumption in the administrative areas, as well as
the production of wastewater and waste from these areas. In addition, environmental loads
associated with the construction and maintenance of infrastructure and equipment (capital
goods) were excluded.
Assumptions and limitations: The results of the environmental impacts and other indicators presented in this EPD refer to
the year 2022.
Quality and other characteristics The quality of the inventory data was assessed taking into account the criteria of the PEF
of the information used in the LCA: (Product Environmental Footprint) category rules (section 5.6 of the guide, Menfredi et al.,
2012), as indicated in table E.2 (Data quality and criteria from the Product Environmental
Footprint Category Rules) of EN 15804:2012+A2:2019+AC and in the guide to the software
used, the GCCA EPD Tool for Cement and Concrete (V 4.2), and based on the
recommendations of the PCR documents - Base Model. The quality of the data was broadly
classified between reasonable and good on a 5-level qualitative scale from very bad to very
good, in line with the data quality requirements - temporal, geographical and technological.
The information on the production of Portland clinker is less than 5 years old, using mostly
primary data collected directly from SECIL - Outão Plant.
For the operations associated with the Portland clinker manufacturing process, real data
specific to the production unit was used. The information for background processes not
provided by SECIL, and over which SECIL has no influence, was obtained from generic data in
the Ecoinvent databasev3.5. These were selected to provide geographical and technological
coverage that fulfils the data quality criteria stipulated in Annex E of EN
15804:2012+A2:2019. Electricity production was modelled on the GCCA, considering the
energy matrix of year 2022, based on data from the International Energy Agency (IEA).
Allocation rules: To determine the inputs and outputs associated only with the production of clinker, the
procedure for subdividing the unit process was first adopted. Thus, only the operations
associated with the production of the product being analysed were considered, and
operations exclusive to other products were excluded. Then, an allocation procedure was
applied for the operations included based on the mass of the different products produced.
The Portland clinker production process also involves multifunctionality associated with the
consumption of waste from other industries as secondary raw materials (e.g. concrete
sludge, calcination residues, lime sludge, kiln linings, construction and demolition waste,
etc.) and secondary fuels (fuels derived from waste, used tyres, etc.), so the environmental
impacts associated with these raw materials and fuels only concern the operations that take
place from their transport to the Outão plant. On the other hand, waste is produced that
will later be recovered, for which further processing has been considered up to the point at
which it is expected to reach end-of-waste status.
Software used for the assessment: GCCA EPD Tool for Cement and Concrete (V 4.2), International version.
Background database used Ecoinvent database version 3.5 published in December 2018; cut-off approach.
for the LCA:
Variability of the results of LCIA The composition of raw materials can also slightly affect the results of the LCIA. The mix of
fuels in the clinker kiln shows a variability of less than 10 per cent in the LCIA results.
Comparability of EPD construction EPD for construction products and services may not be comparable if they are not produced
products': in accordance with EN 15804 and EN 15942 and in accordance with the comparability
conditions determined by ISO 14025.
DAPHabitat System
5
1.10. Use of average environmental performance
Not applicable
1.11. Technical information for Reference Service Life (RSL)
Not applicable
1.12. Diagram of the process input and output flows
Figure 1: Flowchart of the Portland clinker manufacturing process.
DAPHabitat System
6
2. CORE ENVIRONMENTAL IMPACT INDICATORS
2.1. Description of the system boundaries
(✓= included; ND = module not declared)
PRODUCT CONSTRUCTI USE STAGE END OF LIFE ENVIRONMENTAL
STAGE ON PROCESS STAGE BENEFITS AND
STAGE BURDENS BEYOND
THE SYSTEM
BOUNDARY
s
s la ir e t a m w Ra t r o p s n a r T r u t c a f u n ag Mn i t r o p s n a r T
s e c o r p
n o it a lla ts n i d n a n o it c u r ts
n
o
C
e s U e c n a n e tn ia M g n ir ia p e R tn e m e c a lp e R n o it a r o ts e R e s u y g r e n e la n o it a r e p O e s u r e t a w la n o it a r e p O d n a n o it
cn uo ri tt si nlo
om c ee Dd t r o p s n a r T g n is s e c o r p e ts a W la s o p s iD
g n ilc y
c e r la itn e t o p ,y r e v o c e r ,e
s
u
e R
A1 A2 A3 A4 A5 B1 B2 B3 B4 B5 B6 B7 C1 C2 C3 C4 D
✓ ✓ ✓ ND ND ND ND ND ND ND ND ND ND ND ND ND ND
The module A1-A3 (product stage) of Portland clinker considers the extraction and processing of primary (natural) raw materials, the
production of secondary raw materials, the transport of raw materials, additives, fuels and electricity to the production unit, the manufacture
of Portland clinker, as well as the processing of waste up to the end of its waste status or its final destination.
The raw material then enters the kiln, moving along the kiln due to its rotation and slight inclination, continuing to heat up and carrying out the
physical-chemical reactions of the clinker process at a temperature of up to 1450ºC, to ultimately obtain clinker. As firing is an energy-intensive
stage, primary fuels are used, i.e. fossil fuels, as well as secondary fuels (fuels derived from waste, e.g. used tyres, fluff - the non-recyclable
textile component of tyres and refuse-derived fuels).
The main raw materials used to produce Portland clinker are marl and limestone, which are extracted in quarries. Mining is carried out above
ground, on plateaus, starting at the highest level.
Once the materials are extracted, they are in the form of blocks measuring up to 1m3, so it is necessary to reduce their size to a dimension
compatible with the transportation, storage and supply of the subsequent manufacturing phases; this operation is performed in the crusher
(hammer crusher). The extracted material is transported by dump-truck to the crusher. At this stage, secondary raw materials are added to the
marl.
This is followed by raw milling, in which the natural and secondary raw materials (materials derived from waste, e.g. concrete sludge,
calcination waste, lime sludge, kiln linings, construction and demolition waste) are subjected to a drying, milling and homogenising process.
Once the proportion of raw materials has been defined, they are transported to mills where the "flour" or “raw” material is produced, i.e. a
finely ground mixture, in well-defined proportions, of all the natural and secondary raw materials. The mill works by injecting water to stabilise
the grinding track layer. The water will mix with the raw materials creating a layer height necessary for the grinding process to be efficient. The
hot gases coming from the kiln will feed the mill, which will cause some of the water to evaporate, making it necessary to replace it (make-up).
This make-up therefore corresponds to actual water consumption. This water comes from the company boreholes and requires treatment with
sodium hypochlorite, sodium chloride, bio-dispersant, chlorine and disinfectant to eliminate bacteria and prevent calcification in the
equipment, respectively. During milling, the "raw" material is also dried, using the heat contained in the exhaust gases from the rotary kilns.
This is followed by the preheating stage in which the raw material is extracted from the storage silos and fed into the preheating system
(cyclone tower), where it is heated by the exhaust gases resulting from the burning of the fuels in the rotary kiln.
From 1450ºC onwards, the clinker begins to cool, still inside the kiln, and is completed in the cooler, where counter-current air is introduced,
using this heated air as secondary and tertiary firing air. This air is generated by the cooler's fans
DAPHabitat System
7
and is therefore divided into secondary air, which goes into the kiln, and tertiary air, which is the air needed for combustion in the calciner. In
this way, there is a partial recovery of the clinker's thermal content to reduce energy consumption in the kilns.
Finally, the clinker is stored for later use in the production of ordinary cement or other hydraulic binders. The transport of clinker to the mills or
for sale is carried out with bag filters to minimise diffuse dust emissions.
Portland clinker is produced ‘dry’, which means that little water is used throughout the production process, with only water being consumed in
the mill, as mentioned above, and irrigation water in the quarry. During the spring/summer months, the quarry paths are watered an average
of 2 times a day (100 m3/day), while during the autumn/winter months they are watered an average of 4 times a day (50 m3/day). The water
used to irrigate the quarry paths and the mill comes from the company boreholes and requires treatment with sodium hypochlorite and sodium
chloride to eliminate bacteria and prevent calcification in the equipment, respectively.
The diesel used for internal movements at the Secil plant and quarry comes from diesel refuelling stations at the plant and quarry. Therefore,
pollutant emissions to rainwater from hydrocarbon separators associated with the diesel refuelling station and the collection of oily water
throughout the plant and in the quarry, associated with the workshop and diesel refuelling station, were considered. The diesel consumption of
emergency generators and the pumping unit was also considered to guarantee the normal operation of clinker production processes in the
event of a temporary power cut.
The transport and treatment of waste resulting from the clinker production process, such as waste containing hydrocarbons, was considered.
2.1.1. Justification for the exemption to declare modules C1, C2, C3, C4 and D
Portland clinker, being an intermediate product, fulfils all the conditions required by EN 15804:2012+A2:2019+AC and EN 16908:2017+A1, to consider
the cradle-to-gate life cycle (A1-A3), namely:
▪ clinker is physically integrated into cement, which does not allow the physical separation of clinker and cement at the end of its life;
▪ the physical and chemical transformation process that clinker undergoes throughout its life cycle means that at the end of its life this
material is not identifiable;
▪ the clinker does not contain biogenic carbon.
DAPHabitat System
8
2.2. Basic environmental impact indicators
Global Global Global warming
Global Depletion
warming warming potential - Land
warming potential of the Acidification
potential - potential - use and land
potential - stratospheric potential;
total; fossil fuels; use change;
biogenic; ozone-layer;
AP
GWP-total GWP-fossil GWP-luluc
GWP-biogenic ODP
Unit kg CO2 eq. kg CO2 eq. kg CO2 eq. kg CO2 eq. kg CFC 11 eq. mol H+ eq.
Module A1-A3 8.57E+02 8.57E+02 4.71E-02 5.39E-02 1.39E-05 1.36E+00
LEGEND:
Product Stage
Units expressed per declared unit (1000 kg Portland clinker).
Eutrophicati Abiotic Abiotic
Eutrophicati Formation Water (user)
on potential Terrestrial depletion depletion
on potential potential deprivation
of aquatic eutrophicati potential potential
of aquatic tropospheric potential;
freshwater; on for non- for fossil
marine; ozone
potential; fossil resources;
formation; WDP
EP- resources;
EP-marine
freshwater EP-terrestrial ADP-fossil
POCP
ADP-
minerals &
metals
m3 eq. of water
Unit kg P eq. kg N eq. mol N eq. Kg COVNM eq. kg Sb eq. MJ, P.C.I globally
unavailable
Module A1-A3 6.94E-03 7.24E-04 5.12E+00 1.37E+00 1.19E-04 3.20E+03 2.34E+01
LEGEND:
Product Stage
Units expressed per declared unit (1000 kg Portland clinker).
The results obtained for the indicators “Abiotic depletion potential for non-fossil resources (ADP-minerals&metals)”, “Abiotic depletion potential for fossil
resources potential (ADP-fossil)” and “Water (user) deprivation potential (WDP)” should be used with caution since the uncertainties associated with them are
high or there is little experience with the indicator
DAPHabitat System
9
2.3. Additional environmental impact indicators
Potential Potential Potential
Potential Potential Potential soil
human Comparative Comparative
incidence of Comparative quality index
exposure Human Toxicity Human Toxicity
disease due to Toxic Unit for
efficiency in Unit, carcinogenic Unit, non-
emissions of fine ecosystems SQP
relation to carcinogenic
particulate matter
U235 HTP-c
PM ETP-fw
HTP-nc
IRP
Incidence
Unit kBq U 235 eq. CTUe CTUh CTUh -
of disease
Module A1-A3 1.76E-05 4.48E+00 4.93E+01 9.86E-07 1.56E-05 1.28E+03
LEGEND:
Product Stage
Units expressed per declared unit (1000 kg Portland clinker).
The impact indicator “potential human exposure efficiency relative to U235” focuses mainly on the possible impact of a low dose of ionising radiation on
human health resulting from the nuclear fuel cycle. It does not consider effects arising from possible nuclear accidents, occupational exposure or the disposal
of radioactive waste in underground facilities. Potential ionising radiation from soil, radon and some building materials is also not measured by this indicator.
The results of the indicators “potential comparative toxic unit for ecosystems (ETP-fw)”, “potential comparative toxic unit for humans, cancer effects”, “potential
comparative toxic unit for humans, not cancer effects” and “potential soil quality index” should be used with caution as the uncertainties associated with them
are high or there is little experience with the indicator.
DAPHabitat System
10
2.4. Indicators describing the utilisation of resources
Primary energy
EPR RR TRR EPNR RNR TRNR
Unit MJ, P.C.I MJ, P.C.I MJ, P.C.I MJ, P.C.I MJ, P.C.I MJ, P.C.I
Module A1-A3 8.74E+02 0.00E+00 8.74E+02 3.20E+03 0.00E+00 3.20E+03
LEGEND:
Product Stage
Units expressed per declared unit (1000 kg Portland clinker).
EPR = use of renewable primary energy excluding renewable primary energy resources used as raw materials; RR = use of renewable primary energy resources
used as raw materials; TRR = total use of renewable primary energy resources (EPR + RR); EPNR = use of non-renewable primary energy excluding non-renewable
primary energy resources used as raw materials; RNR = use of non-renewable primary energy resources used as raw materials; TRNR = total use of non-
renewable primary energy resources (EPRN + RNR).
Secondary material and fuel, and water use
Net value of fresh
SM RSF NRSF
water
Unit kg MJ, P.C.I MJ, P.C.I m3
Module A1-A3 8.25E+01 3.17E+02 8.50E+02 6.10E-01
LEGEND:
Product Stage
Units expressed per declared unit (1000 kg Portland clinker).
SM = use of secondary material; RSF= use of renewable secondary fuels; NRSF = use of non-renewable secondary fuels; Fresh water = use of the net value of fresh
water.
2.5. Other environmental information describing different categories of waste
Non-hazardous waste
Hazardous waste disposed Radioactive waste disposed
disposed
Unit kg kg kg
Module A1-A3 2.10E-01 1.43E-03 0.00+00
LEGEND:
Product Stage
Units expressed per declared unit (1000 kg Portland clinker).
The characteristics that make waste hazardous are described in the applicable legislation in force, for example in the European Waste Framework Directive.
DAPHabitat System
11
2.6. Other environmental information describing output flows
Components Materials Materials for Exported energy
for reuse for energy
recycling recovery
Unit kg kg kg MJ
Module A1-A3 0.00E+00 2.06E+00 9.20E+00 0.00E+00
LEGEND:
Product Stage
Units expressed per declared unit (1000 kg Portland clinker).
The characteristics that make waste hazardous are described in the applicable legislation in force, for example in the European Waste Framework Directive.
2.7. Information describing the biogenic carbon content at the plant gate
Biogenic carbon content* Units** Module A1-A3 (results)
Biogenic carbon content in the product Kg C Not applicable
Biogenic carbon content in the packaging Kg C Not applicable
* 1 kg of biogenic carbon is equivalent to 44/12 kg of CO2
** This information may be omitted when the biogenic carbon content of the product or its packaging is less than 5 per cent of the mass of the
product or its packaging.
DAPHabitat System
12
3. REFERENCES
✓ GCCA (2023). GCCA Industry EPD Tool for cement and concrete (V4.0). Global Cement and Concrete Association
(GCCA) Quantis, Switzerland;
✓ DAPHabitat System General Instructions, Version 2.1, August 2023 (at www.daphabitat.pt);
✓ PCR - Base Model. Construction products and services. In accordance with EN 15804:2012+A2:2019.
DAPHabitat System. Version 2.3, August 2023 (at www.daphabitat.pt);
✓ NP ISO 14025:2009 Environmental labelling and declarations - Type III environmental declarations - Principles
and procedures;
✓ EN 15804:2012+A2:2019+AC Sustainability of construction works - Environmental product declarations - Core
rules for the product category of construction products;
✓ EN 16908:2017+A1 - Cement and building lime - Environmental product declarations - Product category rules
complementary to EN 15804 European Committee for Standardisation;
✓ EN 15942:2021 Sustainability of construction works – Environmental product declarations – Communication
format business-to-business;
✓ Manfredi S., Allacker K., Chomkhamsri K., Pelletier N., Maia de Souza D. (2012). Product Environmental
Footprint (PEF) Guide. European Commission (EC), Joint Research Centre (JRC), Ispra, Italy;
✓ Secil (2023). Secil CO2 Manual. Monitoring, calculating and reporting CO2 emissions. Period 2021-2025. Version
06.
DAPHabitat System
13
