Applicant's logo]
DAPHabitat System Environmental Product Declaration
www.daphabitat.pt [ACCORDING TO ISO 14025, EN 15804:2012+A2:2019 and EN 15942]
Registration number: DAP 004:2024
CEM II/B-M (V-L) 42.5R COMPOSITE PORTLAND CEMENT- MACEIRA-LIZ
Issue date: 2024-05-20 VALID UNTIL: 2029-05-19
SECIL – COMPANHIA GERAL DE CAL E CIMENTO, S.A.
Product image
Maximum dimensions: 9.40 cm x 16.75 cm
Note: if the dimensions of the image do not correspond to the desired dimensions, it will have to be processed.
The product image may be smaller than specified.
Version 1.4.1. Ed. March 2024
Index
1. GENERAL INFORMATION ................................................................................................................. 1
1.1. The DAPHabitat System .............................................................................................................................. 1
1.2. EPD Owner ................................................................................................................................................... 1
1.3. Information concerning the EPD ................................................................................................................. 2
1.4. Demonstration of the verification .............................................................................................................. 2
1.5. EPD Registration .......................................................................................................................................... 2
1.6. PCR (product category rules) basic model .................................................................................................. 3
1.7. Relevant c-PCR (Complementary product category rules) ......................................................................... 3
1.8. Information concerning the product/product class ................................................................................... 4
1.9. Calculation rules of the LCA ........................................................................................................................ 5
1.10. Use of average environmental performance ............................................................................................. 6
1.11. Technical information for Reference Service Life (RSL) ............................................................................. 6
1.12. Flow diagram of input and output of the processes .................................................................................. 7
2. CORE ENVIRONMENTAL IMPACT INDICATORS............................................................................... 8
2.1. Description of the system boundaries ........................................................................................................ 8
2.1.1. Justification for the exemption to declare modules C1, C2, C3, C4 and D................................................. 9
2.2. Core environmental impact indicators ..................................................................................................... 10
2.3. Additional environmental impact indicators ........................................................................................... 11
2.4. Indicators describing the utilisation of resources .................................................................................... 12
2.5. Other environmental information describing different waste categories .............................................. 12
2.6. Other environmental information describing output flows .................................................................... 13
2.7. Information describing the biogenic carbon content at the factory gate ............................................... 13
3. REFERENCES ................................................................................................................................... 14
DAPHabitat System
iii
1. GENERAL INFORMATION
1.1. The DAPHabitat System
Platform for Sustainable Construction Association
Programme operator: www.centrohabitat.net
centrohabitat@centrohabitat.net
Departamento Engenharia Civil
Address: Universidade de Aveiro
3810-193 Aveiro
Email address: deptecnico@centrohabitat.net
Telephone number: (+351) 234 401 576
Website: www.daphabitat.pt
Logo:
1.2. EPD Owner
Name of the owner: SECIL - Companhia Geral de Cal e Cimento, S.A.
Production site: Fábrica Maceira-Liz
2405-019, Maceira-Leiria
Address (head office): Estrada do Outão, s/n
2901-864 Setúbal
Telephone: (+351) 217 927 100
Email address: apoiotecnico@secil.pt
Website: https://www.secil.pt/
Logo:
Information concerning the NP EN ISO 9001 - Quality Management System
NP ISO 14001 - Environmental Management System
applicable management
ISO 45001 - Health and Safety Management System
systems: EMAS | Eco-Management Audit Scheme
Specific aspects regarding the CAE (economic activity code) 23510 - Manufacture of cement
production:
Organisation’s environmental Commitments made by SECIL as part of its Environmental Responsibility and Protection
policy:
policy:
• To ensure a responsible performance standard that makes using natural
resources compatible with the maintenance and development of the ecosystems
in which the company operates.
• To mitigate the impacts of its actions, through adopting the best technologies and
best practices available and the appropriate training of its employees.
• To promote biodiversity in the territories under its management. To reduce the
carbon impact of its activity, including by promoting the use of secondary raw
materials and alternative fuels.
To provide the public with regular data on its environmental performance.
DAPHabitat System
1
1.3. Information concerning the EPD
Authors: Paula Quinteiro
Secil - Companhia Geral de Cal e Cimento, S.A.
Authors’ contact: Address: Universidade de Aveiro, Campus Universitário de Santiago, 3810-193 Aveiro,
Portugal
Telephone: 234 370 200
E-mail: p.sofia@ua.pt
Address: Estrada do Outão s/n, 2901-864 Setúbal, Portugal
E-mail: info.pssg@secil.pt
Issue date: 20/05/2024
Registration date: 31/05/2024
Registration number: DAP 004:2024
Valid until: 19/05/2029
Representativity of the EPD
EDP of one (1) product class, produced in one (1) industrial unit, belonging to one (1) single
(location, product, group of
producer (Secil - Companhia Geral de Cal e Cimento, S.A)
producers):
Where to consult product https://www.secil.pt
information:
Type of EPD Cradle-to-gate EPD (A1-A3)
1.4. Demonstration of the verification
Independent external verification in accordance with the NP ISO 14025:2010 and EN 15804:2012+A2:2019 standards
Certification Body Verifier (s)
(CERTIF – Associação para a Certificação) (Marisa Almeida | José Dinis Silvestre)
1.5. EPD Registration
Programme Operator
(Platform for Sustainable Construction)
DAPHabitat System
2
1.6. PCR (product category rules) basic model
Name: Base PCR model for construction products and services
Issue date: Edition August 2023
Number of registration on the database: RCP-mb001
Version: Version 2.3
Identification and contact details of the Marisa Almeida | marisa@ctcv.pt
coordinator(s): Luís Arroja | arroja@ua.pt
José Dinis Silvestre | jose.silvestre@ist.utl.pt
Marisa Almeida | marisa@ctcv.pt
Identification and contact of the
Luís Arroja | arroja@ua.pt
authors: José Silvestre | jds@civil.ist.utl.pt
Fausto Freire
Cristina Rocha
Ana Paula Duarte
Ana Cláudia Dias
Helena Gervásio
Victor Ferreira
Ricardo Mateus
António Baio Dias
Composition of the sector panel: -
Consultation period: 18/11/2015 - 18/01/2016
Valid until: 01/06/2027
The CEN EN 15804 standard serves as the core Product Category Rules (PCR).
1.7. Relevant c-PCR (Complementary product category rules)
Name: EN 16908:2017+A1:2022 - Cement and building lime - Environmental product
declarations - Product category rules complementary to EN 15804
Issue date: March 2022
Number of registration on the dataset: EN 16908:2017+A1:2022 E
Version: EN 16908:2017+A1, March 2022
Identification and contact of the European Committee for Standardisation (CEN)
coordinator(s):
Identification and contact of the -
authors:
Composition of the sector panel: -
Consultation period: -
Valid until: -
DAPHabitat System
3
1.8. Information concerning the product/product class
Identification of the product: CEM II/B-M (V-L) 42,5R composite Portland cement
Illustration of the product:
Brief description of the product: CEM II/B-M (V-L) 42.5R composite Portland cement is a product with good chemical
resistance, produced mainly from Portland clinker - with a composition of 65%-79%
Portland clinker, 21%-35% fly ash and limestone, 0%-5% minority constituents. Most of
the clinker comes from SECIL - Maceira-Liz Plant.
CEM II/B-M (V-L) 42.5R composite Portland cement is a highly versatile product that can
be used in various situations and types of concrete and mortar.
The cement does not contain any substance included on the Candidate List of Substances
of Very High Concern (SVHC) above the limit for registration with the European Chemicals
Agency, i.e. above 0.1 per cent (m/m).
Main technical characteristics of the
Table 1: Chemical, mechanical and physical characteristics of CEM II/B-M (V-L) 42.5R
product:
composite Portland cement.
Units Standards
CEM II/B-M (V-L)
Designation 42,5R Portland
Cement
Sulphate Content (in SO3) % ≤ 4.0 NP EN 196-2
Chloride Content % ≤ 0.10 NP EN 196-2
First days: NP EN 196-1
2 days: ≥ 20
Compressive strength MPa 7 days: -
Reference: 28 days,
≥ 42.5 and ≤ 62.5
Start of setting min ≤ 60 NP EN 196-3
Expandability min ≤ 10 NP EN 196-3
Description of the product´s application CEM II/B-M (V-L) 42.5R composite Portland cement is used in:
use: ▪ direct and indirect foundations, tunnels, tanks and other elements in moderately
to very aggressive environments (water or soils rich in harmful salts);
▪ medium and high-strength ready-mixed or site-made structural concrete;
▪ industrial pavements and surfaces subject to chemical attack;
▪ shotcrete, lightweight concrete and blinding concrete;
▪ lightweight high turnover prefabrication;
▪ concrete for road floors, bases and wear layers;
▪ soil treatment and stabilisation, jetgrouting.
Placing on the market/Rules for NP EN 197-1: Composition, specifications and conformity criteria for ordinary cements
application in the market/Technical Conformity Certification
product standards:
Quality control: Not applicable
Special delivery conditions: Not applicable
Components and substances to declare: Not applicable
Where explanatory material may be CEM II/B-M (V-L) 42.5R composite Portland cement is not available for sale to the general
public.
obtained: For detailed information on the product, please contact SECIL at info.pssg@secil.pt.
History of LCA studies: -
DAPHabitat System
4
1.9. Calculation rules of the LCA
Functional unit: Not applicable
Declared unit: 1000 kg of CEM II/B-M (V-L) 42.5R composite Portland cement
System boundaries: The system evaluated includes the A1-A3 module (product stage). A more detailed
description of the system boundary is given in Section 2.1.
Criteria for the exclusion: The LCA considered the extraction and processing of natural raw materials, the transport of
clinker from Algeria to the Secil Maceira plant, the transport of secondary raw materials
(bottom ash and gypsum forms), the production of auxiliary materials and the energy
consumed in the manufacture of CEM II/B-M (V-L) 42.5R composite Portland cement. As the
Portland clinker produced at Secil is the main raw material, the extraction and processing of
natural raw materials and the transport of secondary raw materials (waste from other
industries) were also taken into account. The waste management processes generated in
the production of clinker (until the end of waste status is reached) for which inventory data
is available were considered.
In Portland clinker, bag filters, refractory lining for rotary kilns, lubricating oils, and
acetylene used in maintenance operations (welding), which individually correspond to a
mass of less than 1% of the total mass of inputs, were excluded from the system boundary.
In the Portland cement compound CEM II/B-M (V-L) 42.5R, grinding bodies were also
excluded because correspond to a mass of less than 1% of the total mass of the inputs in
module A1-A3. The total mass of input from the unit processes does not exceed 5% of the
total mass of inputs in module A1-, and is therefore covered by the exclusion criterion
defined in document EN 16908:2017+A1 - Cement and building lime - Environmental
product declarations - Product category rules, namely its mass is less than 1% of the total
mass of inputs
In the LCA for Portland cement, it should be noted that the energy and water consumption
of the administrative areas, as well as the production of wastewater and waste from these
areas, were not included. In addition, environmental loads associated with the construction
and maintenance of infrastructure and equipment (capital goods) were excluded.
Assumptions and limitations: The results of the environmental impacts and other indicators presented in this EPD refer to
the period between May 2022 and June 2023
Quality and other characteristics of the The quality of the inventory data was assessed taking into account the criteria of the PEF
(Product Environmental Footprint) category rules (section 5.6 of the guide, Menfredi et al.,
information used in the LCA: 2012), as indicated in table E.2 (Data quality and criteria from the Product Environmental
Footprint Category Rules) of EN 15804:2012+A2:2019+AC and in the guide to the software
used, the GCCA EPD Tool for Cement and Concrete (V 4.0), and based on the
recommendations of the PCR documents - Base Model. The quality of the data was broadly
classified between reasonable and good on a 5-level qualitative scale from very bad to very
good, in line with the data quality requirements - temporal, geographical and technological.
The information on the production of II/B-M (V-L) 42.5R Portland Cement is less than 5
years old, using mostly primary data collected directly from SECIL - Maceira - Liz Plant.
Real and specific data from the production unit was used for the operations associated with
the process of manufacturing II/B-M (V-L) 42.5R Portland cement. The information for
background processes not provided by SECIL, and over which SECIL has no influence, was
obtained from generic data in the Ecoinvent databasev3.5. These were selected to provide
geographical and technological coverage that fulfils the data quality criteria stipulated in
Annex E of EN 15804:2012+A2:2019.
Electricity production was modelled in the GCCA with information obtained from SECIL’s
electricity producer and supplier.
Allocation rules: To determine the inputs and outputs associated only with the production of CEM II/B-M (V-
L) 42.5R composite Portland cement, the procedure for subdividing the unit process was
first adopted, following the recommendations of the PCR - Base Model document. Thus,
only the operations associated with the production of the product being analysed were
taken into account, and operations exclusive to other products were excluded. Then, for
the operations included, an allocation procedure was applied based on the mass of the
different products produced.
In the production process of CEM II/B-M (V-L) 42.5R Portland cement, forms of gypsum
(secondary raw material) are consumed, i.e. the recovery of waste from external suppliers.
In this case of waste recovery, the "Cut-off" approach was adopted, which is compatible
with EN 16908:2017+A1 and the PCR Base Model document.
Software used for the assessment: GCCA EPD Tool for Cement and Concrete (V 4.0), International version
Background database used for the LCA: Ecoinvent database version 3.5 published in December 2018; cut-off approach.
DAPHabitat System
5
Variability of the results of LCIA: The main factor affecting the variability of LCIA results will be the clinker content used in the
production of CEM II/B-M (V-L) 42.5R composite Portland cement, which can vary from 69%
to 76%, with the average clinker consumption being 73%. This variability in cement
composition resulted in a variability of less than 10 per cent in the LCIA results.
When assessing the possibility of clinker produced in Algeria being produced at SECIL-
Maceira-Liz, there was a variability of less than 15 per cent in the LCIA results.
Comparability of EPD for construction EPD for construction products and services may not be comparable if they are not produced
following EN 15804 and EN 15942 and following the comparability conditions determined by
products' EPD: ISO 14025.
1.10. Use of average environmental performance
Not applicable
1.11. Technical information for Reference Service Life (RSL)
Not applicable
DAPHabitat System
6
1.12. Flow diagram of input and output of the processes
Figure 1: Flowchart of the manufacturing process for CEM II/B-M (V-L) 42.5R Portland cement
DAPHabitat System
7
2. CORE ENVIRONMENTAL IMPACT INDICATORS
2.1. Description of the system boundaries
(✓= included; ND = module not declared)
PRODUCT CONSTRUCTI USE STAGE END OF LIFE STAGE BENEFITS AND LOAD
STAGE ON PROCESS BEYOND THE SYSTEM
STAGE BOUNDARY
s la ir e t a m w Ra t r o p s n a r T g n ir u t c a fu n a M t r o p s n a r T s s e c o r p n o it a lla ts n i n o it c u r ts
n
o
e s U e c n a n e tn ia M r ia p e R tn e m e c a lp e R tn e m h s ib r eu Rf e s u y g r e n e la n o it a r e p O e s u r e t a w la n o it a r e p O n on io t cit uil ro tsm n ee o Dd c -, t r o p s n a r T g n is s e c o r p e ts a W la s o p s iD g n ilc y c e r ,y r e v o c
ela
ri t ,en se ut o p
C e
R
A1 A2 A3 A4 A5 B1 B2 B3 B4 B5 B6 B7 C1 C2 C3 C4 D
✓ ✓ ✓ ND ND ND ND ND ND ND ND ND ND ND ND ND ND
Module A1-A3 (product stage) of CEM II/B-M (V-L) 42.5R composite Portland cement takes into account the extraction and processing of
primary (natural) raw materials, the production of secondary raw materials, the transport of raw materials, additives, fuels and electricity to the
production unit, and the manufacture of CEM II/B-M (V-L) 42.5R composite Portland cement.
The production of CEM II/B-M (V-L) 42.5Rcomposite Portland cement requires clinker, gypsum and limestone as the main raw materials. Most
of the clinker, 90 per cent, used to produce CEM II/B-M (V-L) 42.5R Portland cement is produced at SECIL's Maceira plant. The rest of the clinker
used to produce the cement in question comes from Secil Pataias (3 per cent), Secil Outão (2 per cent) and clinker from Algeria (5 per cent).
The limestone comes from quarries. Mining is carried out above ground, on plateaus, starting at the highest level. The plaster comes from
external production.
The main raw materials used to produce Secil Portland clinker are marl or clay and limestone. Once the materials are extracted from the quarry,
they are in the form of blocks measuring up to 1m3, so it is necessary to reduce their size to a dimension compatible with the transportation,
storage and supply of the subsequent manufacturing phases; this operation is performed in the crusher. After crushing, the natural raw
materials are stored, which is combined with a pre-homogenisation function so that the various uniform stockpiles. This is followed by raw
milling, in which the natural and secondary raw materials (materials derived from waste, e.g. foundry sands, ceramic shards, calcium carbonate
sludge, construction and demolition waste, used refractory bricks) are subjected to a drying, milling and homogenising process. Once the
proportion of raw materials has been defined, they are transported to mills where the "flour" or “raw” material is produced, i.e. a finely ground
mixture, in well-defined proportions, of all the natural and secondary raw materials. At this stage, the raw material is dried using the heat
contained in the exhaust gases from the rotary kilns. This is followed by the preheating stage in which the raw material is extracted from the
storage silos and fed into the preheating system (cyclone tower), where it is heated by the exhaust gases resulting from the burning of the fuels
in the rotary kiln.
The raw material then enters the kiln, moving along the kiln due to its rotation and slight inclination, continuing to heat up and carrying out the
physical-chemical reactions of the clinker process at a temperature of up to 1450ºC, to ultimately obtain clinker. As firing is an energy-intensive
stage, primary fuels are used, i.e. fossil fuels, as well as secondary fuels (fuels derived from waste, e.g. used tyres, fluff and fuels derived from
waste).
DAPHabitat System
8
From 1450ºC onwards, the clinker begins to cool, still inside the kiln, and is completed in the cooler, where counter-current air is introduced,
using this heated air as secondary firing air. In this way, there is a partial recovery of the clinker's thermal content to reduce energy
consumption in the kilns. Particle matter emissions are controlled by dedusting systems and gas emissions into the air by automated control
systems for driving the furnaces. The firing phase produces a powder that comes from a bypass of the gaseous effluent to remove chlorides
from the raw material and fuels, which are then treated by a bag filter. This bypass powder is a by-product, partly sold and partly consumed
internally in cement production (used as a component in cement mills).
The clinker is stored and then used to produce CEM II/B-M (V-L) 42.5R Portland cement. The transport of clinker to the mills is carried out with
bag filters to minimise diffuse dust emissions.
The cement is then produced in horizontal tubular mills. The clinker, gypsum (cement setting regulator), limestone and the other constituents
are ground (e.g. bottom ash, gypsum moulds, grinding aid, chromium reducer) in defined proportions, according to the quality plan, to obtain
CEM II/B-M (V-L) 42.5R composite Portland cement, which is stored in silos. The cement is ground in a closed-circuit using 3rd generation
separators. Also, to minimise diffuse dust emissions, the cement mill has bag filters. Spot monitoring of total suspended particulate emissions is
carried out.
CEM II/B-M (V-L) 42.5R Composite Portland cement is sold in bulk in a tank to the group’s company.
The LCA considered the consumption of electricity, gases and lubricating oils (in the case of clinker production), as well as internal movements
in transport screens, for example, the transport of crushed natural materials to the warehouse.
Just like the production of Portland clinker, cement is produced by the 'dry process' is very small However, during the production of Portland
clinker, water is consumed through evaporation in the cooling towers that go to the clinker kiln's bag filter. This water comes from our own
boreholes and requires treatment with sodium hypochlorite and sodium chloride.
During clinker production, diesel is used for internal movements at Secil. This diesel comes from a diesel refuelling station at the plant. In
clinker production, pollutant emissions to rainwater from the hydrocarbon separators associated with the diesel refuelling station and the
collection of oily water throughout the plant were therefore taken into account. The diesel consumption of emergency generators was also
taken into account in order to guarantee the normal operation of clinker production processes in the event of a temporary power cut. The
transport and treatment of waste resulting from the clinker production process, such as waste containing hydrocarbons, was considered.
The production of CEM II/B-M (V-L) 42.5R composite Portland cement and its subsequent sale in bulk does not result in the generation of
waste.
2.1.1. Justification for the exemption to declare modules C1, C2, C3, C4 and D
CEM II/B-M (V-L) 42.5R composite Portland cement fulfils all the conditions required by EN 15804:2012+A2:2019+AC, EN 16908:2017+A1, to
consider the life cycle from cradle-to-gate (module A1-A3), namely:
▪ cement is physically integrated into concrete, which means that cement and concrete cannot be physically separated at the end of
life;
▪ the physical and chemical transformation process that cement undergoes throughout its life cycle means that at the end of its life
this material is not identifiable;
▪ the cement does not contain biogenic carbon.
DAPHabitat System
9
2.2. Core environmental impact indicators
Global Global Global warming Global warming Depletion
warming warming potential land use potential of the Acidification
potential
potential potential and land use stratospheric potential;
biogenic;
total; fossil change; ozone layer;
AP
GWP-total GWP-fossil GWP-biogenic GWP-luluc ODP
Unit kg CO2 eq. kg CO2 eq. kg CO2 eq. kg CO2 eq. kg CFC 11 eq. mol H+ eq.
Module A1-A3 6.53+02 6.53+02 6.27-02 7.11-02 1.46-05 1.57E+00
LEGEND:
Product stage
Units expressed per declared unit (1000 kg cement CEM II/B-M (V-L) 42.5R Portland cement ).
Eutrophication Abiotic Abiotic
p ao qt uen att ii ca l Eu ptr oo tp eh nic ta iati lo n Eu ptr oo tp eh nic ta iati lo n pF oo tr em na tit aio
l
on
f
pod te ep nle tit aio
l
fn
o r
pod te ep nle tit aio
l
fn
o r
W dea pte rir
v
( au ts ioe nr)
aquatic tropospheric non-fossil fossil
freshwater; terrestrial; potential;
marine; ozone; resources; resources
potential;
EP- EP-terrestrial WDP
EP-marine POCP ADP-
freshwater minerals&metals ADP-fossil
m3 World eq.
Unit kg P eq. kg N eq. mol N eq. Kg COVNM eq. kg Sb eq. MJ, P.C.I
deprived
Module A1-A3 2.27E-02 1.72E-03 5.10E+00 1.24E+00 2.23E-04 2.56E+03 2.73E+01
LEGEND:
Product stage
P.C.I. – Net calorific value
Units expressed per declared unit (1000 kg cement CEM II/B-M (V-L) 42.5R Portland cement).
The results obtained for the indicators “Abiotic depletion potential for non-fossil resources (ADP-minerals&metals)”, “Abiotic depletion potential for fossil resources
potential (ADP-fossil)” and “Water (user) deprivation potential (WDP)” should be used with caution since the uncertainties associated with them are high or there is
little experience with the indicator.
DAPHabitat System
10
2.3. Additional environmental impact indicators
Potential Potential
Potential Potential Potential
incidence of Human Comparative
Comparative Comparative Toxic Potential soil
disease due exposure Toxic Unit for
Toxic Unit for Unit for humans, quality index
to PM efficiency humans, not
ecosystems cancer effects
emissions relative to U235 cancer effects SQP
IRP ETP-fw HTP-c
PM HTP-nc
Incidence of
Unit kBq U 235 eq. CTUe CTUh CTUh -
disease
Module A1-A3 3.24E-05 8.91E+03 8.20E+01 1.67E-06 3.46E-05 1.34E+03
Legend:
Product stage
P.C.I. – Net calorific value
Units expressed per declared unit (1000 kg cement CEM II/B-M (V-L) 42.5R Portland cement).
The life cycle stages (or scenarios) not considered in the study can be eliminated of the table, through the function “eliminate lines” .
The impact indicator “potential human exposure efficiency relative to U235” focuses mainly on the possible impact of a low dose of ionising radiation on human
health resulting from the nuclear fuel cycle. It does not consider effects arising from possible nuclear accidents, occupational exposure or the disposal of
radioactive waste in underground facilities. Potential ionising radiation from soil, radon and some building materials is also not measured by this indicator.
The results of the indicators “potential comparative toxic unit for ecosystems (ETP-fw)”, “potential comparative toxic unit for humans, cancer effects”,
“potential comparative toxic unit for humans, not cancer effects” and “potential soil quality index” should be used with caution as the uncertainties associated
with them are high or there is little experience with the indicator.
DAPHabitat System
11
2.4. Indicators describing the utilisation of resources
Primary energy
EPR RR TRR EPNR RNR TRNR
Unit MJ, P.C.I MJ, P.C.I MJ, P.C.I MJ, P.C.I MJ, P.C.I MJ, P.C.I
Module A1-A3 2.09+02 0.00E+00 2.09+02 2.56E+03 0.00E+00 2.56E+03
LEGEND:
Product stage
Units expressed per declared unit (1000 kg cement CEM II/B-M (V-L) 42.5R Portland cement).
EPR = use of renewable primary energy excluding renewable primary energy resources used as raw materials; RR = use of renewable primary energy resources
used as raw materials; TRR = total use of renewable primary energy resources (EPR + RR); EPNR = use of non-renewable primary energy excluding non-
renewable primary energy resources used as raw materials; RNR = use of non-renewable primary energy resources used as raw materials; TRNR = total use of
non-renewable primary energy resources (EPRN + RNR);
Secondary material and fuel, and water use
MS CSR CSNR Net use of fresh water
Unit kg MJ, P.C.I MJ, P.C.I m3
Module A1-A3 2.15E+02 4.59E+02 6.12+02 7.14E-01
LEGEND:
Product Stage
Units expressed per declared unit (1000 kg cement CEM II/B-M (V-L) 42.5R Portland cement).
S = use of secondary material; CSR = use of renewable secondary fuels; CSNR = use of non-renewable secondary fuels.
2.5. Other environmental information describing different waste categories
Hazardous waste disposed Non-hazardous waste disposed Radioactive waste disposed
Unit kg kg kg
Module A1-A3 3.95E-01 1.24-02 0,00+00
LEGEND:
Product stage
Units expressed per declared unit (1000 kg cement CEM II/B-M (V-L) 42.5R Portland cement).
The characteristics that make waste hazardous are described in the applicable legislation in force, for example in the European Waste Framework Directive.
DAPHabitat System
12
2.6. Other environmental information describing output flows
Materials for Exported energy
Components for Materials for
recycling
reuse energy recovery
Unit kg kg kg MJ
Module A1-A3 0.00E+00 3.34E-01 2.84E-01 0.00E+00
LEGEND
Product stage
Units expressed per declared unit (1000 kg cement CEM II/B-M (V-L) 42.5R Portland cement).
The characteristics that make waste hazardous are described in the applicable legislation in force, for example in the European Waste Framework Directive.
2.7. Information describing the biogenic carbon content at the factory gate
Biogenic carbon content* Units** Modules A1-A3 (results)
Biogenic carbon content in the product Kg C 0
Biogenic carbon content in accompanying packaging Kg C 0
* 1 kg biogenic carbon is equivalent to 44/12 kg of CO2.
** This information can be omitted whenever the content of biogenic carbon in the product, or in the respective packaging, is less than 5% of the
mass of the product, or the respective packaging.
DAPHabitat System
13
3. REFERENCES
✓ GCCA (2023). GCCA Industry EPD Tool for cement and concrete (V4.0). Global Cement and Concrete Association
(GCCA) Quantis, Switzerland.
✓ DAPHabitat System General Instructions, Version 2.0, June 2022 (at www.daphabitat.pt).
✓ NP ISO 14025:2009 Environmental labelling and declarations - Type III environmental declarations - Principles
and procedures.
✓ EN 15804:2012+A2:2019+AC Sustainability of construction works - Environmental product declarations - Core
rules for the product category of construction products.
✓ EN 16908:2017+A1 - Cement and building lime - Environmental product declarations - Product category rules
complementary to EN 15804 European Committee for Standardisation.
✓ EN 15942:2021 Sustainability of construction works – Environmental product declarations – Communication
format business-to-business.
✓ Manfredi S., Allacker K., Chomkhamsri K., Pelletier N., Maia de Souza D. (2012). Product Environmental
Footprint (PEF) Guide. European Commission (EC), Joint Research Centre (JRC), Ispra, Italy.
✓ PCR - Base model for construction products and services DAPHabitat System. Version 2.3, 2023 (at
www.daphabitat.pt).
✓ Secil (2023). Secil CO Manual. Monitoring, calculating and reporting CO emissions. Period 2021-2025. Version
2 2
06.
DAPHabitat System
14
