ENVIRONMENTAL PRODUCT DECLARATION
as per ISO 14025 and EN 15804+A2
Owner of the Declaration DuPont de Nemours (Luxembourg) s.à.r.l.
Programme holder Institut Bauen und Umwelt e.V. (IBU)
Publisher Institut Bauen und Umwelt e.V. (IBU)
Declaration number EPD-DUP-20220252-CBA1-EN
Issue date 16.11.2022
Valid to 15.11.2027
DuPontTM Tyvek® laminated 2528B
DuPont de Nemours (Luxembourg) s.à.r.l.
www.ibu-epd.com | https://epd-online.com
Umwelt Produktdeklaration Name des Herstellers – Name des Produkts
General Information
DuPont de Nemours (Luxembourg) s.à.r.l. DuPontTM Tyvek® laminated 2528B
Programme holder Owner of the declaration
IBU – Institut Bauen und Umwelt e.V. DuPont de Nemours (Luxembourg) s.à.r.l.
Hegelplatz 1 Rue Général Patton
10117 Berlin L-2984 Contern
Germany Luxembourg
Declaration number Declared product / declared unit
EPD-DUP-20220252-CBA1-EN 1 m2 DuPontTM Tyvek® laminated 2528B
This declaration is based on the product Scope:
category rules: This document applies to DuPontTM Tyvek® laminated
False ceiling and underlay sheeting, 11.2017 2528B, which is a laminated high-density polyethylene
(PCR checked and approved by the SVR) (HDPE) membrane with spunbond polypropylene
(SBPP). The declared unit weight is 206 g/m2. LCA
data were compiled using production data for the year
Issue date
2019 for monolayer, lamination and finishing processes
16.11.2022
(used for EPDs of Tyvek® laminated published in
2021) and data for the year 2021 for the SBPP
Valid to production. The declaration holder is responsible for
15.11.2027 the underlying data and its verification.
The owner of the declaration shall be liable for the
underlying information and evidence; the IBU shall not
be liable with respect to manufacturer information, life
cycle assessment data and evidences.
The EPD was created according to the specifications
of EN 15804+A2. In the following, the standard will be
simplified as EN 15804.
Verification
The standard EN 15804 serves as the core PCR
Independent verification of the declaration and data
according to ISO 14025:2011
Dipl. Ing. Hans Peters internally x externally
(chairman of Institut Bauen und Umwelt e.V.)
Dr. Alexander Röder Vito D'Incognito
(Managing Director Institut Bauen und Umwelt e.V.)) (Independent verifier)
Product
Product description/Product definition For the application and use the respective national
DuPont™ Tyvek® 2528B is a durable, water-resistant provisions apply.
membrane that is reinforced with a laminated
polypropylene nonwoven. This vapour-permeable Application
membrane is extremely water-resistant and can be The product is placed in front or behind insulation and
used for all supported and unsupported pitched roofs. will improve water and wind tightness during
construction and the lifetime of the building.
For the placing on the market of the product in the
European Union/European Free Trade Association Technical Data
(EU/EFTA) (with the exception of Switzerland)
Regulation (EU) No. 305/2011 (CPR) applies.
Constructional data (nominal or average values)
The product needs a declaration of performance taking Name Value Unit
into consideration EN 13859-1 Flexible sheets for Reaction to fire acc. to EN13501-1 E* class
waterproofing - Definitions and characteristics of Grammage acc. to EN 1849-2 0.206 kg/m2
underlays - Part 1: Underlays for discontinuous roofing Resistance to water penetration
W1 -
and EN 13859-2 Part 2: Underlays for walls. acc. to EN 1928 (class)
Water vapor diffusion equivalent
For the placing on the market of the product in the UK air layer thickness acc. to EN 0.03 m
market the product needs UK Conformity Assessed 12572 (C)
(UKCA) marking supported by a UK Approved Body.
2 Environmental Product Declaration DuPont de Nemours (s.à r.l.) – DuPont™ Tyvek® laminated (2528B)
Resistance to air penetration acc. m3/m2 h
0 - 2
to EN 12114 50Pa Base materials/Ancillary materials
Maximum tensile force acc. to EN The product is made from HDPE (ca. 39 % of product
275 - 275 N/50mm
12311-1 (MD-XD) weight), SBPP (ca. 53 % of product weight) and
Elongation acc. to EN 12311-1 ethylene vinyl acetate (ca. 7 % of product weight).
13 - 20 %
(MD-XD)
Tear Resistance (nail) acc. to EN This product/article/at least one partial article contains
36 - 41 N/mm
12310-1 (MD-XD) substances listed in the candidate list (date: 16. Nov
Maximum tensile force after 2022) exceeding 0.1 percentage by mass: no.
ageing acc. to EN 1297, EN 202 - 202 N/50mm
12311-1 (MD-XD) Reference service life
Elongation after ageing acc. to EN The service life of membranes out of plastic or
1297, EN 12311-1 (MD-XD) 9 - 11 % elastomers is 40 years according to BNB
(http://www.nachhaltigesbauen.de/baustoff-und-
Resistance to water penetration
gebaeudedaten/nutzungsdauern-von-bauteilen.html).
after ageing acc. to EN 1297, EN W1 -
Since the whole lifecycle of the product is not
1928 (class)
considered and for sake of compliance with EN
*on mineral wool and wood
15804+A2 (2019), the functional unit does not have to
be declared. Instead, the declaration unit is 1 m2 of the
 Performance data of the product in
envelope.
accordance with the declaration of
performance with respect to its essential
characteristics according to Application:
Flexible sheets for water proofing – Part 2:
Underlays for walls EN 13859-2:2010
LCA: Calculation rules
Declared Unit
This declaration applies to 1 m2 of DuPont™ Tyvek® The representativeness can be classified as very good
2528B membrane, with a declared unit weight of 206 for all the foreground data, and for most of the
g/m2. background data.
Declared unit The GaBi database (Sphera Solutions GmbH, 2022.1)
Name Value Unit was used to model background data.
Declared unit 1 m2
Grammage 0.206 kg/m2
System boundary
Primary production data were collected to model the Type of EPD: Cradle-to-gate (with options)
four production steps for manufacturing (A1-A3). The system boundaries of the EPD follow the modular
Manufacturing data are representative for the years construction system as described by EN 15804.
2019 and 2021; the product is manufactured in The LCA considers the following modules:
Luxembourg and Germany. All energy and materials  A1-A3: Manufacturing of pre-products,
flows were considered. Only a few material flows were packaging, ancillary materials, transport to the
excluded from the modelling, but the sum of their factory and production, with the associated
weight did not exceed 1 % of the total input mass.
energy supply and waste handling
Manufacturing of the production machines and
 A4: Transport to the construction site
systems and associated infrastructure were not taken
into account for the life cycle assessment.  A5: Installation into the building including
disposal of packaging
Transport to the construction site (A4) were based on  C4: Waste disposal, namely incineration
market shares of 2021 at country level, provided by
 D: Potential for reuse, recovery and/or
DuPont Luxembourg s.à.r.l., to cover at least 90 % of
recycling including benefits for product
sales. Eurostat data representative of 2019 were used
to model the shares between the packaging disposal incineration from module C4
routes during the installation into the building (A5).
Regarding possible off-cuts during installation, the
amount is lower than 5 % and therefore neglected. Comparability
Basically, a comparison or an evaluation of EPD data
Regarding background data, the Luxembourg and is only possible if all the data sets to be compared
German electricity grid mix were applied to the were created according to EN 15804 and the building
production plants in these countries. Other background context, respectively the product-specific
data were specific to Germany or the European characteristics of performance, are taken into account.
average and were not older than 10 years. A proxy
was used for the colour paste for finishing (generic
water-based colour paste composition).
LCA: Scenarios and additional technical information
Characteristic product properties
3 Environmental Product Declaration DuPont de Nemours (s.à r.l.) – DuPont™ Tyvek® laminated (2528B)
Information on biogenic carbon
The product does not contain biogenic carbon.
Information on describing the biogenic Carbon
Content at factory gate
Name Value Unit
Biogenic Carbon Content in
0 kg C
product
Biogenic Carbon Content in
0.0037 kg C
accompanying packaging
Transport to the building site (A4)
Name Value Unit
Transport distance (truck) 502 km
Transport distance (container ship) 0 km
Installation into the building (A5)
Name Value Unit
Wood waste to landfill 2.74E-04 kg
Wood waste to incineration 2.26E-04 kg
Cardboard waste to landfill 2.66E-04 kg
Cardboard waste to incineration 2.84E-04 kg
Plastic waste to landfill 2.47E-05 kg
Plastic waste to incineration 3.94E-05 kg
End of life (C1-C4)
Name Value Unit
Collected separately Tyvek®
0.206 kg
waste
Energy recovery 0.206 kg
4 Environmental Product Declaration DuPont de Nemours (s.à r.l.) – DuPont™ Tyvek® laminated (2528B)
LCA: Results
The results displayed below apply to 1 m2 of DuPont™ Tyvek® laminated 2528B membrane, with a declared unit
weight of 206 g/m2.
DESCRIPTION OF THE SYSTEM BOUNDARY (X = INCLUDED IN LCA; ND = MODULE OR INDICATOR NOT
DECLARED; MNR = MODULE NOT RELEVANT)
BENEFITS AND
CONSTRUCTI LOADS
PRODUCT STAGE ON PROCESS USE STAGE END OF LIFE STAGE BEYOND THE
STAGE SYSTEM
BOUNDARIES
5 Environmental Product Declaration DuPont de Nemours (s.à r.l.) – DuPont™ Tyvek® laminated (2528B)
lairetam
waR
ylppus tropsnarT
gnirutcafunaM
eht
morf
tropsnarT
etis
eht
ot
etag
ylbmessA esU
ecnanetniaM
riapeR
tnemecalpeR tnemhsibrufeR
ygrene
lanoitarepO esu
retaw
lanoitarepO esu
noitcurtsnoc-eD
noitilomed tropsnarT
gnissecorp
etsaW
lasopsiD -esueR -yrevoceR -gnilcyceR laitnetop
A1 A2 A3 A4 A5 B1 B2 B3 B4 B5 B6 B7 C1 C2 C3 C4 D
X X X X X ND ND MNR MNR MNR ND ND ND ND ND X X
RESULTS OF THE LCA - ENVIRONMENTAL IMPACT according to EN 15804+A2: 1 m2 DuPont™ Tyvek®
2528B
Core Indicator Unit A1-A3 A4 A5 C4 D
Global warming potential - total [kg CO2-Eq.] 9.74E-1 8.94E-3 1.93E-3 6.65E-1 -3.89E-1
Global warming potential - fossil fuels [kg CO2-Eq.] 9.69E-1 8.74E-3 1.56E-4 6.65E-1 -3.87E-1
Global warming potential - biogenic [kg CO2-Eq.] 4.45E-3 1.46E-4 1.77E-3 -3.93E-5 -1.47E-3
GWP from land use and land use change [kg CO2-Eq.] 2.18E-4 4.97E-5 2.32E-8 0.00E+0 -2.92E-5
Depletion potential of the stratospheric ozone layer [kg CFC11-Eq.] 9.10E-12 5.34E-16 1.47E-16 4.38E-10 -1.58E-12
Acidification potential, accumulated exceedance [mol H+-Eq.] 4.62E-3 5.31E-5 4.00E-7 8.75E-5 -3.92E-4
Eutrophication, fraction of nutrients reaching freshwater
[kg P-Eq.] 1.29E-5 2.66E-8 3.35E-9 1.59E-9 -3.30E-7
end compartment
Eutrophication, fraction of nutrients reaching marine end
[kg N-Eq.] 6.97E-4 2.61E-5 1.70E-7 1.50E-5 -1.20E-4
compartment
Eutrophication, accumulated exceedance [mol N-Eq.] 7.53E-3 2.88E-4 1.65E-6 3.49E-4 -1.30E-3
Formation potential of tropospheric ozone photochemical
[kg NMVOC-Eq.] 2.18E-3 4.93E-5 6.67E-7 4.38E-5 -3.42E-4
oxidants
Abiotic depletion potential for non-fossil resources [kg Sb-Eq.] 1.07E-7 7.45E-10 5.05E-12 9.35E-15 -4.24E-8
Abiotic depletion potential for fossil resources [MJ] 2.25E+1 1.19E-1 8.11E-4 1.25E-1 -6.43E+0
Water (user) deprivation potential, deprivation-weighted [m³ world-Eq
2.15E-1 8.00E-5 1.05E-4 5.84E-2 -2.48E-2
water consumption (WDP) deprived]
RESULTS OF THE LCA - INDICATORS TO DESCRIBE RESOURCE USE according to EN 15804+A2: 1 m2
DuPont™ Tyvek® 2528B
Indicator Unit A1-A3 A4 A5 C4 D
Renewable primary energy as energy carrier [MJ] 2.05E+0 6.77E-3 1.03E-4 3.24E-3 -1.09E+0
Renewable primary energy resources as material utilization [MJ] 1.56E-3 3.61E-14 6.33E-15 3.84E-6 -8.29E-11
Total use of renewable primary energy resources [MJ] 2.06E+0 6.77E-3 1.03E-4 3.24E-3 -1.09E+0
Non-renewable primary energy as energy carrier [MJ] 2.25E+1 1.19E-1 8.12E-4 1.25E-1 -6.43E+0
Non-renewable primary energy as material utilization [MJ] 4.63E-4 4.19E-6 1.74E-8 3.69E-10 -1.51E-4
Total use of non-renewable primary energy resources [MJ] 2.25E+1 1.19E-1 8.12E-4 1.25E-1 -6.43E+0
Use of secondary material [kg] 7.74E-3 0.00E+0 0.00E+0 0.00E+0 0.00E+0
Use of renewable secondary fuels [MJ] 1.85E-6 0.00E+0 0.00E+0 0.00E+0 0.00E+0
Use of non-renewable secondary fuels [MJ] 1.85E-6 0.00E+0 0.00E+0 0.00E+0 0.00E+0
Use of net fresh water [m³] 9.13E-3 7.66E-6 2.49E-6 1.36E-3 -1.05E-3
RESULTS OF THE LCA – WASTE CATEGORIES AND OUTPUT FLOWS according to EN 15804+A2:
1 m2 DuPont™ Tyvek® 2528B
Indicator Unit A1-A3 A4 A5 C4 D
Hazardous waste disposed [kg] 3.70E-8 5.72E-13 1.11E-13 0.00E+0 -9.89E-10
Non-hazardous waste disposed [kg] 5.49E-3 1.71E-5 4.11E-4 0.00E+0 -2.57E-3
Radioactive waste disposed [kg] 3.55E-4 1.47E-7 2.01E-8 7.09E-6 -3.10E-4
Components for re-use [kg] 0.00 0.00 0.00 0.00 0.00
Materials for recycling [kg] 0.00 0.00 0.00 0.00 0.00
Materials for energy recovery [kg] 0.00 0.00 0.00 0.00 0.00
Exported electrical energy [MJ] 0.00E+0 0.00E+0 1.38E-3 9.76E-1 0.00E+0
Exported thermal energy [MJ] 0.00E+0 0.00E+0 2.49E-3 3.21E+0 0.00E+0
RESULTS OF THE LCA – additional impact categories according to EN 15804+A2-optional:
1 m2 DuPont™ Tyvek® 2528B
Indicator Unit A1-A3 A4 A5 C4 D
Potential incidence of disease due to PM emissions [Disease
ND ND ND ND ND
Incidence]
Potential Human exposure efficiency relative to U235 [kBq U235-
ND ND ND ND ND
Eq.]
Potential comparative toxic unit for ecosystems [CTUe] ND ND ND ND ND
Potential comparative toxic unit for humans - cancerogenic [CTUh] ND ND ND ND ND
Potential comparative toxic unit for humans - not cancerogenic [CTUh] ND ND ND ND ND
Potential soil quality index [-] ND ND ND ND ND
Disclaimer 1 – for the indicator “Potential Human exposure efficiency relative to U235”.
This impact category deals mainly with the eventual impact of low-dose ionizing radiation on human health of the
nuclear fuel cycle. It does not consider effects due to possible nuclear accidents, occupational exposure or
radioactive waste disposal in underground facilities. Potential ionizing radiation from the soil, radon and from
some construction materials is also not measured by this indicator.
Disclaimer 2 – for the indicators “abiotic depletion potential for non-fossil resources”, “abiotic depletion potential
for fossil resources”, “water (user) deprivation potential, deprivation-weighted water consumption”, “potential
comparative toxic unit for ecosystems”, “potential comparative toxic unit for humans – cancerogenic”, “Potential
comparative toxic unit for humans - not cancerogenic”, “potential soil quality index”.
The results of this environmental impact indicator shall be used with care as the uncertainties on these results are
high as there is limited experience with the indicator.
References
Standards
EN 15804
EN 12114 EN 15804:2012+A2:2019+AC:2021, Sustainability of
EN 12114:2000, Thermal performance of buildings - construction works — Environmental Product
Air permeability of building components and building Declarations — Core rules for the product category of
elements - Laboratory test method construction products.
EN 12310-1 EN 1849-2
EN 12310-1:1999, Flexible sheets for waterproofing - EN 1849-2:2019, Flexible sheets for waterproofing -
Part 1: Bitumen sheets for roof waterproofing; Determination of thickness and mass per unit area -
determination of resistance to tearing (nail shank). Part 2: Plastic and rubber sheets
EN 12311-1 EN 1928
EN 12311-1:1999, Flexible sheets for waterproofing - EN 1928:2000, Flexible sheets for waterproofing -
Part 1: Bitumen sheets for roof waterproofing; Bitumen, plastic and rubber sheets for roof
Determination of tensile properties waterproofing - Determination of watertightness
EN 12572 ISO 14025
EN 12572:2016, Hygrothermal performance of building EN ISO 14025:2011, Environmental labels and
materials and products — Determination of water declarations — Type III environmental declarations —
vapour transmission properties — Cup method Principles and procedures.
EN 1297 Further References
EN 1297:2004, Flexible sheets for waterproofing -
Bitumen, plastic and rubber sheets for roof BNB
waterproofing - Method of artificial ageing by long term Bewertungssystem Nachhaltiges Bauen
exposure to the combination of UV radiation, elevated https://www.nachhaltigesbauen.de/austausch/nutzungs
temperature and water dauern-von-bauteilen/
EN 13501-1 GaBi software and database:2022
EN 13501-1:2018. Fire classification of construction GaBi software/database, version 10.6.1.35. Sphera
products and building elements - Part 1: Classification Solutions GmbH, 2022.
using data from reaction to fire tests
IBU 2021
EN 13859-1 Institut Bauen und Umwelt e.V.: General Instructions
EN 13859-1:2014, Flexible sheets for waterproofing - for the EPD programme of Institut Bauen und Umwelt
Definitions and characteristics of underlays - Part 1: e.V., Version 2.0, Berlin: Institut Bauen und Umwelt
Underlays for discontinuous roofing e.V., 2021. www.ibu-epd.com
EN 13859-2 PCR 2021, Part A
EN 13859-2:2014, Flexible sheets for waterproofing - PCR Guidance-Texts for Building-Related Products
Definitions and characteristics of underlays - Part 2: and Services: Calculation Rules for the Life Cycle
Underlays for walls
6 Environmental Product Declaration DuPont de Nemours (s.à r.l.) – DuPont™ Tyvek® laminated (2528B)
Assessment and Requirements on the Project Report DuPont™, the DuPont Oval Logo, and all trademarks
according to EN 15804+A2:2019 and service marks denoted with ™, SM or ® are
owned by affiliates of DuPont de Nemours, Inc. unless
PCR 2017, Part B otherwise noted.
PCR Guidance-Texts for Building-Related Products
and Services: Requirements on the EPD for False
ceiling and underlay sheeting (version 1.6, 2017)
7 Environmental Product Declaration DuPont de Nemours (s.à r.l.) – DuPont™ Tyvek® laminated (2528B)
Publisher
Institut Bauen und Umwelt e.V. Tel +49 (0)30 3087748- 0
Hegelplatz 1 Fax +49 (0)30 3087748- 29
10117 Berlin Mail info@ibu-epd.com
Germany Web www.ibu-epd.com
Programme holder
Institut Bauen und Umwelt e.V. Tel +49 (0)30 - 3087748- 0
Hegelplatz 1 Fax +49 (0)30 – 3087748 - 29
10117 Berlin Mail info@ibu-epd.com
Germany Web www.ibu-epd.com
Author of the Life Cycle
Assessment Tel 00352-275888-1
Luxembourg Institute of Science Fax 00352-275888-555
and Technology (LIST) Mail info@list.lu
Avenue des Hauts-Fourneaux 5 Web www.list.lu
4362 Esch/Alzette
Luxembourg
Owner of the Declaration
DuPont de Nemours (Luxembourg) Tel +352 3666 5210
s.à r.l. Fax +352 3666 0000
Rue Général Patton 1 Mail tyvek.info@dupont.com
2984 Contern Web www.dupont.com
Luxembourg
