ENVIRONMENTAL PRODUCT DECLARATION
as per ISO 14025 and EN 15804+A2
Owner of the Declaration
Programme holder Institut Bauen und Umwelt e.V. (IBU)
Publisher Institut Bauen und Umwelt e.V. (IBU)
Declaration number EPD­ZIN­20210262­IBG1­EN
Issue date 22.03.2022
Valid to 21.03.2027
duroZINQ® hot-dip galvanized steel
ZINQ Technologie GmbH
www.ibu-epd.com | https://epd-online.com
Umwelt Produktdeklaration Name des Herstellers – Name des Produkts
1. General Information
ZINQ Technologie GmbH duroZINQ® hot­dip galvanized steel
Programme holder Owner of the declaration
IBU – Institut Bauen und Umwelt e.V. ZINQ Technologie GmbH
Panoramastr. 1 An den Schleusen 6
10178 Berlin 45881 Gelsenkirchen
Germany Deutschland
Declaration number Declared product / declared unit
EPD­ZIN­20210262­IBG1­EN 1 t of duroZINQ® hot­dip galvanized structural steel
This declaration is based on the product Scope:
category rules: This EPD refers to 1t of duroZINQ® hot­dip galvanized
Structural steels, 11.2017 steel galvanized at facilities of the ZINQ® group (see
(PCR checked and approved by the SVR) www.zinq.com/standorte). Representative foreground
data from five duroZINQ® hot­dip galvanizing plants
collected by ZINQ Technologie GmbH and background
Issue date
data from the GaBi database was used to conduct the
22.03.2022
LCA study. The data were weighted according to the
yearly production and the galvanized surface area of
Valid to the products.
21.03.2027
The owner of the declaration shall be liable for the
underlying information and evidence; the IBU shall not
be liable with respect to manufacturer information, life
cycle assessment data and evidences.
The EPD was created according to the specifications
of EN 15804+A2. In the following, the standard will be
simplified as EN 15804.
Verification
The standard EN 15804 serves as the core PCR
Independent verification of the declaration and data
according to ISO 14025:2010
Dipl. Ing. Hans Peters internally x externally
(chairman of Institut Bauen und Umwelt e.V.)
Dr. Alexander Röder Matthias Klingler
(Managing Director Institut Bauen und Umwelt e.V.)) (Independent verifier)
2. Product
2.1 Product description/Product definition gathered for this background report is 115.7
This EPD applies to 1 t (1000 kg) of duroZINQ® hot­ µm
dip galvanized structural steel which are products of
ZINQ Technologie GmbH and applied for the purpose
The EPD covers steel products of the grades S235 to
of corrosion protection of said steel components.
S960 rolled out to structural sections, merchant bars
Characteristics are:
and heavy plates with the aforementioned zinc coating.
 Hot­dip zinc coating according to DIN EN ISO
The steel products are manufactured via Blast Furnace
1461 consisting of a zinc layer and
with Basic Oxygen Furnace (BF+BOF) and Electric Arc
intermetallic zinc­iron­phases as a result of
Furnace (EAF) routes according to the EPD of
the hot­dip galvanizing process Structural steel: Sections and plates.
 Applied on steel components, e.g. hot­rolled
sections or structures welded from heavy For the placing on the market of the product in the
European Union/European Free Trade Association
plates; a typical surface of such steel
(EU/EFTA) (with the exception of Switzerland)
components per ton is 15 – 80 m², the
Regulation (EU) No. 305/2011 (CPR) applies. The
average value resulting from the data
product needs a declaration of performance taking into
gathered for this background reports is 40 m² consideration EN 10025-1: 2005 Hot rolled products of
per ton of product structural steels – Part 1: General technical delivery
 Typical zinc coating thickness is 60 – 200 µm, conditions and EN ISO 1461:2009 Hot dip galvanized
coatings on fabricated iron and steel articles ­
the average value resulting from the data
Specifications and test methods and the CE­marking.
2 Environmental Product Declaration ZINQ Technologie GmbH – duroZINQ(R) hot­dip galvanized steel
For the application and use the respective national 2.5 Base materials/Ancillary materials
provisions apply. One ton of the hot­dip galvanized structural steels
covered in this EPD consist of 966.94 kg of structural
2.2 Application steel according to the EPD of Structural steel: Sections
Structural steels are intended for bolted, welded or and plates and 33.06 kg of protective zinc coating. The
otherwise connected constructions of buildings or other masses are based on the declared unit (40 m2
load­bearing (support) structures but also for surface, 115.7 µm coating thickness).
infrastructure components, commercial vehicle
components and other structures. The zinc coatings Materials (zinc & auxiliaries) of the coating process:
applied to steel structures serve in particular the  Primary and secondary (remelted) zinc and
purpose of protecting these against corrosive and/or zinc alloys
mechanical loading during the use phase. They thus
 Industrial cleaner
are applied in steel applications where relevant
 Degreaser
corrosive loadings occur and appropriate protection
against these is required to extend the service life of  Acid degreasing additives
the steel components and ensure their functionality.  Wetting agents
Zinc coatings also serve additional purposes, such as  Pickling additives
optical design and improved fire protection.
 Hydrochloric acid
Examples of hot­dip galvanized steel applications
 Hydrogen peroxide
include:
 Single story buildings like industrial and  Flux (Zinc chloride and Ammonium chloride)
storage halls  Passivation
 Multi­storey buildings like offices, residential  Binding wire
buildings, car parks and shops
 Bridges for different modes of transport like Hot­dip galvanized steel is not a substance or mixture
railway or roads under the chemical law (REACH). Nethertheless, the
following declaration are given for duroZINQ hot­dip
 Sub­structure of solar panels, scaffoldings or
galvanized steel:
shelving systems
 This product/article/at least one partial article
 crash barriers, sign posts and sign bridges
contains substances listed in the candidate
list (date: 18.12.2019) exceeding 0.1
percentage by mass: no
 This product/article/at least one partial article
2.3 Technical Data
contains other CMR substances in categories
This EPD is valid for steel products of varied
grades and different forms of delivery according to the 1A or 1B which are not on the candidate list,
EPD of Structural steel: Sections and plates. exceeding 0.1 percentage by mass: no.
 Biocide products were added to this
Technical Data
construction product or it has been treated
Name Value Unit
with biocide products (this then concerns a
Density 7850 kg/m3
treated product as defined by the (EU)
Modulus of elasticity 210000 N/mm2
Coefficient of thermal expansion 12 10­6K­1 Ordinance on Biocide Products No.
Thermal conductivity 48 ­ 58 W/(mK) 528/2012): no.
Melting point depending on the
1536 °C
alloy up to
2.6 Manufacture
Performance data of the product in accordance with The manufacturing of structural steel refers to the EPD
the declaration of performance with respect to its of Structural steel: Sections and plates.
essential characteristics according to EN 10025, Hot
rolled products of structural steels. Further product In hot­dip galvanizing, the fully or semi­fabricated steel
standards: ASTM A36, ASTM A283, ASTM A514, components are first cleaned using a wet­chemical
ASTM A572, ASTM A573, ASTM A588, ASTM A633, pre­treatment and then coated by dipping them into the
ASTM A709, ASTM A913, ASTM A992 and ASTM molten liquid zinc melt. This includes the use of natural
A1066.For the execution of steel structures EN 1090 gas to fire the molten zinc to ~450°C, ensuring a
has to be taken into consideration. For hot­dip constant temperature and compensating for thermal
galvanizing EN ISO 1461, Hot dip galvanized coatings losses, as well as the drying furnace. Electrical energy
on fabricated iron and steel articles ­ Specifications is used for the extraction system at the galvanizing
and test methods has to be taken into consideration. kettel and for the cranes that move the galvanizing
Further relevant standards: EN ISO 14713-1, EN ISO material through the process. For this purpose, racks,
14713-2, ASTM A123, ASTM A143, ASTM A153, hooks, chains, wires and traverses are used in addition
ASTM A384, ASTM A385. as auxiliary equipment.
2.4 Delivery status 2.7 Environment and health during
The dimensions of the products declared in this EPD manufacturing
may vary depending on the intended application.
During production, there are no special requirements
for safety, environmental protection and health beyond
3 Environmental Product Declaration ZINQ Technologie GmbH – duroZINQ(R) hot­dip galvanized steel
the legal requirements. Compliance with these
requirements is verified in the course of duroZINQ® 2.10 Condition of use
hot­dip galvanizing using management systems (ISO duroZINQ® hot­dip galvanized steel products are non­
14001, ISO 45001 and ISO 50001). In addition, a /low­alloyed steel products with a protective coating,
complete assessment of all substances used in the which results from hot­dip galvanizing in a zinc melt
process and duroZINQ® product, including an ABC­X of at least 98 mass% zinc, the rest being amounts of
analysis, was carried out as part of the Cradle-to- minor alloying elements such as aluminium or
Cradle certification process (certification has been bismuth.
valid continuously since 2013). During use the zinc coatings undergo permanent
reactions with its atmosphere, building a very resistant
zinc carbonate layer (carbonisation). Under ongoing
2.8 Product processing/Installation corrosive loading of the zinc coating the zinc corrodes
and the layer becomes thinner over time. This process
Processing recommendations: of zinc consumption or zinc loss takes place very
Planning, processing, implementation and intended slowly at a zinc corrosion rate. For an average
use of duroZINQ® hot­dip galvanized section and plate corrosive atmosphere, the corrosion rate could be
constructions have to be carried out depending on the assumed to 1.3 µm/year according to EN ISO 12944-2.
respective applications according to the generally
recognized rules of engineering and manufacturer’s
recommendations. The standards of EN 1993 and EN 2.11 Environment and health during use
1994 apply to the design of steel structures and The protective layer of the zinc coating (zinc
composite steel and concrete structures. They include carbonate, patina) formed naturally under the influence
the requirements regarding serviceability, bearing of air and moisture is very stable and not soluble in
capacity, durability and fire resistance of steel water (see 2.10) under consideration of today's
structures EN 1993 and composite steel and concrete strongly reduced air pollution (here especially the SO
2
structures EN 1994. concentration in the air) and proper application (no
EN 1090-1 and EN 1090-2 apply to the execution of water drainage permanently provided by the design).
steel structures and include the requirements for The zinc ion runoff significantly depends on the load of
factory production control. In addition, these European "acidic" air pollutants, especially SO . As the SO
2 2
Standards will work in connection with national concentration in the air has decreased to one­fifth of
amendments, national instructions, guidelines and previous levels over the past 30 years, there has also
publications, as well as legal provisions. been a corresponding decrease in the zinc runoff and
Regarding transport and storage of duroZINQ® hot­dip thus of the zinc concentration in precipitation water.
galvanized sections and plates, the generally accepted The legal limits for the total concentration of zinc in
requirements for securing loads have to be observed. drinking water are undercut. In water systems, only a
Instruction details of the manufacturer based on small portion of the total zinc concentration is available
verified standards and guidelines e.g. regarding to an organism; this amount is called the biologically
welding, bolting, hot and cold forming or assembly are available amount. It is related to the physicochemical
to be observed in every case. conditions of the receiving water body. For example,
bioavailability is affected by the amount of zinc that is
Occupational safety/Environmental protection: organically or inorganically bound, bound to particles,
When processing/using duroZINQ® hot­dip galvanized or competing with other ions.
steel sections and plates pursuant to the generally There are no known adverse effects on health when
recognized rules of engineering there are no measures steel hot­dip galvanized with duroZINQ® is used as
to be taken which are going beyond the public intended. Like iron, zinc is one of the metals essential
occupational health and safety. for life. Zinc is not accumulated in the body. The zinc
The processing/using of duroZINQ® hot­dip galvanized intake recommendation of the German Nutrition
steel sections and plates pursuant to the generally Society (DGE) is 15 mg daily.
recognized rules of engineering does not release
substantial environmental pollutants. Particular 2.12 Reference service life
measures to protect the environment are not required. Structural steel products are supposed to serve at
least the lifetime of a building which is 50 years
Residual material: according to EN 15978. The technical service life of a
During duroZINQ® hot­dip galvanizing as well as galvanized steel product is determined by the time the
during processing of duroZINQ® hot­dip galvanized protecting zinc coating stays on the steel to protect it
steel residual pieces as well as turnings are to be from corrosion. At a rate of 1.3 µm per year (section
separately collected. Zinc­rich waste from the 2.10) this leads to a technical service life of at least 89
duroZINQ® hot­dip galvanizing process is treated and years and therefore exceeds the 50 years lifetime of
returned to the zinc cycle. duroZINQ® hot­dip buildings.
galvanized scrap steel is entirely recycled by melting
and producing new steel products.
Optionally, duroZINQ® hot­dip galvanized steel can be 2.13 Extraordinary effects
returned at its end of life to the ZINQ facility, where the
duroZINQ® coating is removed and the zinc is Fire
reintroduced into the zinc cycle. The material is class A1, i.e. not flammable per EN
13501.
2.9 Packaging Under fire load, the zinc coating has a positive effect
No additional packaging is necessary since on the steel structure in that it slows down its heating,
the duroZINQ® coating provides the protecting which ensures the load­bearing capacity of the
function of a package. structure for a longer period of time compared to
ungalvanized, unprotected steel.
4 Environmental Product Declaration ZINQ Technologie GmbH – duroZINQ(R) hot­dip galvanized steel
When heated above 650°C, the thin zinc coating
evaporates briefly as zinc oxide (ZnO), producing 2.14 Re-use phase
smoke. The ZnO smoke, inhaled over a longer period Steel sections and plates made of duroZINQ® hot­dip
of time, can cause "zinc fever" (diarrhoea, fever, dry galvanized steels are recyclable to 100 % EPD of
throat), which, however, disappears completely some Structural Steel: Sections and Plates. Re­use takes
days after inhalation. place for around 11 % of the products while 88 % are
recycled in a closed loop. Around 1 % can not be
regained due to occurring losses. The zinc coating is
Brandschutz carbonized over the lifetime of the steel structure.
Name Value
Building material class A1 2.15 Disposal
Due to its high value as a raw material, hot­dip
Water galvanized steel scrap is not disposed of but recycled
Under the influence of water, no negative effects on in a long­established cycle. Reaction products of the
the functional capability of duroZINQ hot­dip zinc coating with the atmosphere (zinc carbonate
galvanized steel within the intended service life are to resulting from carbonization) are removed from the
be expected ­ provided that it is used as intended. surface in very low concentrations over the lifespan of
the steel product, but without known harm to the
Mechanical destruction environment.
Due to the ductility of steel and the high mechanical Waste code according to European Waste Catalogue
resistance of the duroZINQ® hot­dip zinc EWC:
coating, duroZINQ® hot­dip steel structures react 17 04 05 ­ iron and steel
resiliently in the event of unforeseeable mechanical
destruction. In case of tensile load necking will occur 2.16 Further information
before cracking. In case of lasting high compression Further information on duroZINQ® products can be
load, components of duroZINQ® hot­dip galvanized obtained from www.zinq.com.
steel may buckle or bulge. No splintering or breaking
edges shall result.
3. LCA: Calculation rules
3.1 Declared Unit For the electricity consumption of the galvanizing
The declared unit is 1t (1000 kg) of hot­dip galvanized process a renewable energy grid mix has been taken
structural steel. Data from 5 representative duroZINQ® into account. The electricity usage of the production of
hot­dip galvanizing sites of the ZINQ® group (see steel, as well as module D refers to to the EPD of
www.zinq.com/standorte) has been used to declare a Structural Steel: Sections and Plates. Electricity credits
representative product (40 m2 surface, 115.7 µm of energy recovery inside the system boundaries have
coating thickness), the total production in 2019 from been accounted for using a German average grid mix.
the 5 sites has been weighted according to the The proportion of green electricity demand for the
galvanized surface and corrected by a factor to galvanizing process is 100%. Therefore, no residual
account for typical products of the respective site. grid mix has been considered.
Declared Unit Module B1-B7 consider the following:
Name Value Unit  Carbonisation of the Zinc coating during use
Declared unit 1 t of the product. This serves as a carbon
dioxide sink. The calculation is based on the
stoichiometric ratio lowered by an amount to
account for real conditions,
3.2 System boundary
Type of the EPD: Cradle to gate with options, modules  during intended use over the considered
C1–C4, and module D. lifetime of hot­dip galvanized structural steels,
Modules A1­A4, B1­B7, C1­C4 and D have been no maintenance, replacement or
considered. refurbishment is needed. The products do not
use energy or water.
Module A1-A4 consider the following:
 Production of structural steel according to the
EPD of Structural Steel: Sections and Plates, Module C1-C4 consider the following:
 Deconstruction of structural steel,
 production of zinc and zinc alloy
 transport to the end­of­life,
components,
 processing and disposal according to the
 transport of the structural steel to the
EPD of Structural Steel: Sections and Plates.
manufacturing sites,
 the galvanizing process, including all
auxiliaries and the use of electricity and Due to carbonisation, no remaining zinc must be
considered.
thermal energy,
 transport from the manufacturing sites to the
Module D considers benefits and loads beyond the
construction site. system boundary according to the EPD of Structural
Steel: Sections and Plates.
5 Environmental Product Declaration ZINQ Technologie GmbH – duroZINQ(R) hot­dip galvanized steel
3.3 Estimates and assumptions
Primary data was used to model all on­site processes 3.5 Background data
of the hot­dip galvanizing process. Data were cross­ The LCA model is created using the GaBi
checked to identify and eliminate data gaps. High­ Software system for life cycle engineering, developed
quality secondary data from the GaBi database was by Sphera Solutions GmbH. The GaBi
used to model upstream material and energy flows. database provides the life cycle inventory data for
Secondary data was as technologically and several of the raw and process materials obtained from
geographically representative as possible. Zn/Al the background system. The most recent of the
master alloys, alloying elements and auxiliaries are database was 2020.
considered using their material weights. Instead of
primary data collection from suppliers to reflect specific 3.6 Data quality
brand products, datasets from the GaBi database for The foreground data collected by ZINQ Technologie
standard processing chemicals have been used. GmbH are based on yearly production amounts in
For sludges, a solid waste content was assumed. This productions plants.
solid waste content is handled as hazardous waste All relevant background datasets are taken from the
with the respective treatment. Waste water and water GaBi database. The study is based on high
content of the sludges are assumed to be treated in quality data.
municipal waste water treatment. Other wastes are
treated as commercial waste in a municipal waste 3.7 Period under review
incineration plant. The foreground data collected by ZINQ Technologie
GmbH are based on yearly production amounts in
productions plants. The production data refer to an
3.4 Cut-off criteria average of the year 2019.
No cut­off criteria are applied in this study. All reported
data were incorporated and modelled using the best 3.8 Allocation
available LCI data. Data for the sites were cross­ Allocation for the structural steel is done according to
checked with one another to identify potential data the EPD of Structural Steel: Sections and Plates. The
gaps. No processes, materials or emissions that are hot­dip galvanizing process does not deliver any co­
known to make a significant contribution to the products. The applied model does not contain any
environmental impact of the products studied have allocation.
been omitted. On this basis, there is no evidence to
suggest that input or outputs contributing more than 1 3.9 Comparability
% to the overall mass or energy of the system or that Basically, a comparison or an evaluation of EPD data
are environmentally significant have been omitted. It is only possible if all the data sets to be compared
can be assumed, that all excluded flows contribute less were created according to EN 15804 and the building
than 5 % to the impact assessment categories. context, respectively the product­specific
Production of capital equipment, facilities and characteristics of performance, are taken into account.
infrastructure required for manufacture are outside the
scope of this assessment. The GaBi database provides the life cycle inventory
Transport of base materials with low shares in the data for several of the raw and process materials
composition are neglected. obtained from the background system. The most
recent of the database was 2020.
4. LCA: Scenarios and additional technical information
Characteristic product properties
Information on biogenic Carbon
The production of the steel refers to the EPD of
Structural Steel: Sections and Plates.
Information for the scenario used is given in the
following tables. Information regarding the service life
is given in section 2.12.
Transport to Construction site (A4)
Name Value Unit
Transport distance 100 km
Capacity utilisation (including
61 %
empty runs)
Ende des Lebenswegs (C1-C4)
Name Value Unit
Reuse 106 kg
Recycling 851 kg
Energy recovery 0 kg
Landfilling 9.67 kg
6 Environmental Product Declaration ZINQ Technologie GmbH – duroZINQ(R) hot­dip galvanized steel
5. LCA: Results
In Table 1 "Description of the system boundary", all declared modules shall be indicated with an "X"; all modules
that are not declared shall be indicated with "MND" (As default the modules B3, B4, B5 are marked as MNR –
module not relevant). In the following tables, columns can be deleted for modules that are not declared. Indicator
values should be declared with three valid digits (eventually using exponential form (e.g. 1,23E­5 = 0,0000123). A
uniform format should be used for all values of one indicator.
If several modules are not declared and therefore have been deleted from the table, the abbreviations for the
indicators can be replaced by the complete names, while the readability and clear arrangement should be
maintained; the legends can then be deleted.
If due to relevant data gaps, an indicator cannot be declared in a robust way, then the abbreviation “IND”
(indicator not declared) should be used for this indicator.
 0 – calculated value is 0
 0 – value falls under the cut­off
 0 – assumption which exclude any flows (e.g. exported electricity A1­A3)
 IND – in cases where the inventory does not support the methodological approach or the calculation of
the specific indicator IND shall be used.
If no reference service life is declared (see chapter 2.13 "Reference Service Life"), the LCA results of the modules
B1­B2 and B6­B7 shall refer to a period of one year. This shall then be indicated as an explanatory text below the
tables. In addition, the formula for the quantification of such B­modules over the total life cycle shall be provided.
Disclaimer:
EP­freshwater: This indicator has been calculated as “kg P eq” as required in the characterization model
(EUTREND model, Struijs et al., 2009b, as implemented in ReCiPe;
http://eplca.jrc.ec.europa.eu/LCDN/developerEF.xhtml).
DESCRIPTION OF THE SYSTEM BOUNDARY (X = INCLUDED IN LCA; ND = MODULE OR INDICATOR NOT
DECLARED; MNR = MODULE NOT RELEVANT)
BENEFITS AND
CONSTRUCTI LOADS
PRODUCT STAGE ON PROCESS USE STAGE END OF LIFE STAGE BEYOND THE
STAGE SYSTEM
BOUNDARIES
7 Environmental Product Declaration ZINQ Technologie GmbH – duroZINQ(R) hot­dip galvanized steel
lairetam
waR
ylppus tropsnarT
gnirutcafunaM
eht
morf
tropsnarT
etis
eht
ot
etag
ylbmessA esU
ecnanetniaM
riapeR
tnemecalpeR tnemhsibrufeR
ygrene
lanoitarepO esu
retaw
lanoitarepO esu
noitcurtsnoc­eD
noitilomed tropsnarT
gnissecorp
etsaW
lasopsiD ­esueR ­yrevoceR ­gnilcyceR laitnetop
A1 A2 A3 A4 A5 B1 B2 B3 B4 B5 B6 B7 C1 C2 C3 C4 D
X X X X ND X X X X X X X X X X X X
RESULTS OF THE LCA - ENVIRONMENTAL IMPACT according to EN 15804+A2: 1 t duroZINQ® hot-dip
galvanized steel
Core Indicator Unit A1 A2 A3 A4 B1 B2 B3 B4 B5 B6 B7 C1 C2 C3 C4 D
­ ­
1.26E+2.91E+8.12E+6.03E+ 0.00E+0.00E+0.00E+0.00E+0.00E+0.00E+1.09E+2.91E+1.73E+0.00E+
GWP­total [kg CO2­Eq.]
3 1 1 0
7.39E+
0 0 0 0 0 0 1 0 0 0
3.68E+
0 2
­ ­
1.25E+2.90E+8.07E+5.99E+ 0.00E+0.00E+0.00E+0.00E+0.00E+0.00E+1.08E+2.90E+1.74E+0.00E+
GWP­fossil [kg CO2­Eq.]
3 1 1 0
7.39E+
0 0 0 0 0 0 1 0 0 0
3.67E+
0 2
6.78E+0.00E+4.41E­0.00E+0.00E+0.00E+0.00E+0.00E+0.00E+0.00E+0.00E+3.60E­0.00E+­1.35E­0.00E+­3.59E­
GWP­biogenic [kg CO2­Eq.]
0 0 1 0 0 0 0 0 0 0 0 2 0 2 0 1
3.51E­ 2.35E­ 3.01E­ 4.86E­0.00E+0.00E+0.00E+0.00E+0.00E+0.00E+0.00E+1.57E­ 2.35E­ 3.13E­0.00E+­2.93E­
GWP­luluc [kg CO2­Eq.]
1 1 2 2 0 0 0 0 0 0 0 2 2 3 0 2
­3.46E­3.49E­ 5.25E­ 7.21E­0.00E+0.00E+0.00E+0.00E+0.00E+0.00E+0.00E+2.38E­ 3.49E­ 3.22E­0.00E+2.74E­
ODP [kg CFC11­Eq.]
7 15 8 16 0 0 0 0 0 0 0 13 16 14 0 13
3.73E+2.98E­­3.25E­6.16E­0.00E+0.00E+0.00E+0.00E+0.00E+0.00E+0.00E+2.39E­ 2.98E­ 4.97E­0.00E+­8.46E­
AP [mol H+­Eq.]
0 2 2 3 0 0 0 0 0 0 0 2 3 3 0 1
6.66E­ 8.82E­ 6.57E­ 1.82E­0.00E+0.00E+0.00E+0.00E+0.00E+0.00E+0.00E+2.89E­ 8.82E­ 4.42E­0.00E+­1.87E­
EP­freshwater [kg P­Eq.]
4 5 5 5 0 0 0 0 0 0 0 5 6 6 0 4
9.47E­ 8.67E­­1.39E­1.79E­0.00E+0.00E+0.00E+0.00E+0.00E+0.00E+0.00E+5.30E­ 8.67E­ 1.32E­0.00E+­1.69E­
EP­marine [kg N­Eq.]
1 3 2 3 0 0 0 0 0 0 0 3 4 3 0 1
­
1.03E+1.04E­­1.38E­2.16E­0.00E+0.00E+0.00E+0.00E+0.00E+0.00E+0.00E+5.57E­ 1.04E­ 1.42E­0.00E+
EP­terrestrial [mol N­Eq.] 1.77E+
1 1 1 2 0 0 0 0 0 0 0 2 2 2 0
0
3.00E+2.41E­ 7.89E­ 4.98E­0.00E+0.00E+0.00E+0.00E+0.00E+0.00E+0.00E+1.45E­ 2.41E­ 3.73E­0.00E+­6.48E­
POCP [kg NMVOC­Eq.]
0 2 2 3 0 0 0 0 0 0 0 2 3 3 0 1
1.80E­ 2.08E­­2.54E­4.30E­0.00E+0.00E+0.00E+0.00E+0.00E+0.00E+0.00E+3.13E­ 2.08E­ 4.42E­0.00E+­3.94E­
ADPE [kg Sb­Eq.]
2 6 3 7 0 0 0 0 0 0 0 6 7 7 0 3
­
1.33E+3.86E+1.31E+7.99E+0.00E+0.00E+0.00E+0.00E+0.00E+0.00E+0.00E+1.90E+3.86E+2.92E+0.00E+
ADPF [MJ] 3.42E+
4 2 3 1 0 0 0 0 0 0 0 2 1 1 0
3
­ ­
[m³ world­Eq 1.38E+2.59E­ 5.37E­0.00E+0.00E+0.00E+0.00E+0.00E+0.00E+0.00E+2.36E+2.59E­ 3.29E­0.00E+
WDP 1.85E+ 3.27E+
deprived] 3 1 2 0 0 0 0 0 0 0 0 2 1 0
2 1
GWP = Global warming potential; ODP = Depletion potential of the stratospheric ozone layer; AP = Acidification potential of land and water; EP =
Caption Eutrophication potential; POCP = Formation potential of tropospheric ozone photochemical oxidants; ADPE = Abiotic depletion potential for non­
fossil resources; ADPF = Abiotic depletion potential for fossil resources; WDP = Water (user) deprivation potential
RESULTS OF THE LCA - INDICATORS TO DESCRIBE RESOURCE USE according to EN 15804+A2: 1 t
duroZINQ® hot-dip galvanized steel
Indicator Unit A1 A2 A3 A4 B1 B2 B3 B4 B5 B6 B7 C1 C2 C3 C4 D
PERE [MJ] 1550.00 21.70 399.00 4.49 0.00 0.00 0.00 0.00 0.00 0.00 0.00 84.30 2.17 11.60 0.00 37.30
PERM [MJ] 0.00 0.00 0.00 0.00 0.00 0.00 0.00 0.00 0.00 0.00 0.00 0.00 0.00 0.00 0.00 0.00
PERT [MJ] 1550.00 21.70 399.00 4.49 0.00 0.00 0.00 0.00 0.00 0.00 0.00 84.30 2.17 11.60 0.00 37.30
13300.0 ­
PENRE [MJ] 387.00 1310.00 80.00 0.00 0.00 0.00 0.00 0.00 0.00 0.00 190.00 38.70 29.20 0.00
0 3420.00
PENRM [MJ] 0.00 0.00 0.00 0.00 0.00 0.00 0.00 0.00 0.00 0.00 0.00 0.00 0.00 0.00 0.00 0.00
13300.0 ­
PENRT [MJ] 387.00 1310.00 80.00 0.00 0.00 0.00 0.00 0.00 0.00 0.00 190.00 38.70 29.20 0.00
0 3420.00
SM [kg] 800.00 0.00 0.00 0.00 0.00 0.00 0.00 0.00 0.00 0.00 0.00 0.00 0.00 0.00 0.00 0.00
RSF [MJ] 0.00 0.00 0.00 0.00 0.00 0.00 0.00 0.00 0.00 0.00 0.00 0.00 0.00 0.00 0.00 0.00
NRSF [MJ] 0.00 0.00 0.00 0.00 0.00 0.00 0.00 0.00 0.00 0.00 0.00 0.00 0.00 0.00 0.00 0.00
FW [m³] 32.50 0.03 ­4.22 0.01 0.00 0.00 0.00 0.00 0.00 0.00 0.00 0.10 0.00 0.01 0.00 ­0.80
PERE = Use of renewable primary energy excluding renewable primary energy resources used as raw materials; PERM = Use of
renewable primary energy resources used as raw materials; PERT = Total use of renewable primary energy resources; PENRE = Use of
non­renewable primary energy excluding non­renewable primary energy resources used as raw materials; PENRM = Use of non­
Caption
renewable primary energy resources used as raw materials; PENRT = Total use of non­renewable primary energy resources; SM = Use
of secondary material; RSF = Use of renewable secondary fuels; NRSF = Use of non­renewable secondary fuels; FW = Use of net fresh
water
RESULTS OF THE LCA – WASTE CATEGORIES AND OUTPUT FLOWS according to EN 15804+A2:
1 t duroZINQ® hot-dip galvanized steel
Indicator Unit A1 A2 A3 A4 B1 B2 B3 B4 B5 B6 B7 C1 C2 C3 C4 D
HWD [kg] 3.52E­41.80E­5­3.31E­53.72E­60.00E+00.00E+00.00E+00.00E+00.00E+00.00E+00.00E+07.87E­81.80E­61.14E­70.00E+0­2.67E­4
NHWD [kg] 17.50 0.06 0.52 0.01 0.00 0.00 0.00 0.00 0.00 0.00 0.00 0.14 0.01 9.70 0.00 24.40
RWD [kg] 6.36E­14.79E­4­6.39E­39.90E­50.00E+00.00E+00.00E+00.00E+00.00E+00.00E+00.00E+02.88E­24.79E­53.86E­30.00E+0­5.85E­2
CRU [kg] 0.00 0.00 0.00 0.00 0.00 0.00 0.00 0.00 0.00 0.00 0.00 0.00 0.00 106.00 0.00 0.00
MFR [kg] 0.00 0.00 0.00 0.00 0.00 0.00 0.00 0.00 0.00 0.00 0.00 0.00 0.00 851.00 0.00 0.00
MER [kg] 0.00 0.00 0.00 0.00 0.00 0.00 0.00 0.00 0.00 0.00 0.00 0.00 0.00 0.00 0.00 0.00
EEE [MJ] 0.00 0.00 0.00 0.00 0.00 0.00 0.00 0.00 0.00 0.00 0.00 0.00 0.00 0.00 0.00 0.00
EET [MJ] 0.00 0.00 0.00 0.00 0.00 0.00 0.00 0.00 0.00 0.00 0.00 0.00 0.00 0.00 0.00 0.00
HWD = Hazardous waste disposed; NHWD = Non­hazardous waste disposed; RWD = Radioactive waste disposed; CRU = Components
Caption for re­use; MFR = Materials for recycling; MER = Materials for energy recovery; EEE = Exported electrical energy; EEE = Exported
thermal energy
RESULTS OF THE LCA – additional impact categories according to EN 15804+A2-optional:
1 t duroZINQ® hot-dip galvanized steel
8 Environmental Product Declaration ZINQ Technologie GmbH – duroZINQ(R) hot­dip galvanized steel
Indicator Unit A1 A2 A3 A4 B1 B2 B3 B4 B5 B6 B7 C1 C2 C3 C4 D
[Disease ­1.41E­ 0.00E+ 0.00E+ 0.00E+ 0.00E+ 0.00E+ 0.00E+ 0.00E+ 0.00E+ ­1.10E­
PM 4.19E­51.77E­7 3.67E­8 2.00E­71.77E­84.87E­8
Incidence] 6 0 0 0 0 0 0 0 0 5
­
[kBq U235­ 1.13E+ ­9.85E­ 0.00E+ 0.00E+ 0.00E+ 0.00E+ 0.00E+ 0.00E+ 0.00E+ 4.73E+ 0.00E+
IRP 6.92E­2 1.43E­2 6.92E­36.32E­1 6.61E+
Eq.] 2 1 0 0 0 0 0 0 0 0 0
0
­ ­
2.14E+ 2.73E+ 5.65E+ 0.00E+ 0.00E+ 0.00E+ 0.00E+ 0.00E+ 0.00E+ 0.00E+ 8.13E+ 2.73E+ 1.36E+ 0.00E+
ETP­fw [CTUe] 2.49E+ 3.04E+
4 2 1 0 0 0 0 0 0 0 1 1 1 0
3 2
­7.31E­ 0.00E+ 0.00E+ 0.00E+ 0.00E+ 0.00E+ 0.00E+ 0.00E+ 5.72E­ 5.01E­ 0.00E+
HTP­c [CTUh] 7.45E­75.72E­9 1.18E­9 2.25E­9 6.45E­8
8 0 0 0 0 0 0 0 10 10 0
­1.00E­ 0.00E+ 0.00E+ 0.00E+ 0.00E+ 0.00E+ 0.00E+ 0.00E+ 0.00E+ ­4.22E­
HTP­nc [CTUh] 4.65E­52.95E­7 6.10E­8 8.27E­82.95E­83.10E­8
6 0 0 0 0 0 0 0 0 6
­
8.04E+ 1.36E+ 7.06E+ 2.80E+ 0.00E+ 0.00E+ 0.00E+ 0.00E+ 0.00E+ 0.00E+ 0.00E+ 6.05E+ 1.36E+ 9.08E+ 0.00E+
SQP [­] 3.22E+
2 2 1 1 0 0 0 0 0 0 0 1 1 0 0
1
PM = Potential incidence of disease due to PM emissions; IR = Potential Human exposure efficiency relative to U235; ETP­fw = Potential
Caption comparative Toxic Unit for ecosystems; HTP­c = Potential comparative Toxic Unit for humans (cancerogenic); HTP­nc = Potential
comparative Toxic Unit for humans (not cancerogenic); SQP = Potential soil quality index
Disclaimer 1 – for the indicator “potential Human exposure efficiency relative to U235“.
This impact category deals mainly with the eventual impact of low dose ionizing
radiation on human health of the nuclear fuel cycle. It does not consider effects due to possible
nuclear accidents, occupational exposure nor radioactive waste disposal in underground
facilities. Potential ionizing radiation from the soil, radon and from some construction materials is also not
measured by this indicator.
Disclaimer 2 – for the indicators: “abiotic depletion potential for fossil resources”, “abiotic depletion potential for
non­fossil resources”, “water (user) deprivation potential”, “deprivation­weighted water consumption”, “potential
comparative toxic unit for ecosystems”, “potential comparative toxic unit for humans ­ cancer effects”, “potential
comparative toxic unit for humans – non­cancer effects”, “potential soil quality index”.
The results of this environmental impact indicator shall be used with care as the
uncertainties on these results are high or as there is limited experience with the indicator.
6. LCA: Interpretation
The interpretation of this EPD highlights the shows the relative contribution of each module for the
contribution of the hot­dip galvanizing process in the different impact categories.
environmental impact of 1 t of duroZINQ® hot­dip Negative contributions of module A3 (the hot­dip
galvanized steel. While the highest share of impacts as galvanizing process) for ADPE and WDP are linked to
for a hot­dip galvanized product is related to the the recovery of high­value zinc, a sulphidic ore, using a
production of the structural steel as part of Module A1, rotary kiln while the upstream of zinc is part of module
this refers to the EPD of Structural Steel: Sections and A1. This results in a net negative value of module A3
Plates. The potential benefits in module D are for impact categories linked to the mining of zinc.
exclusively attributable to the steel. Additionally, the The results show a similar trend to GWP for most of
use phase serves as a sink for CO due to the impact categories Module A1 is linked to the
2
carbonization of the zinc coating. The following graph highest impacts and module D offers benefits to reuse
and recycling of the structural steel.
9 Environmental Product Declaration ZINQ Technologie GmbH – duroZINQ(R) hot­dip galvanized steel
7. Requisite evidence
7.1 Weathering performance load and a coastal atmosphere with low salt load and
The corrosion rate of zinc depends on the position of thus corresponds to the typical corrosive load of steel
the component and the conditions of the surrounding structures, the corrosion rate is assumed to be 1.3
atmosphere (corrosivity categories according to EN µm/year.
ISO 12944-2). For corrosivity category C3, which
according to this standard is characteristic of an urban
and industrial atmosphere with moderate sulfur dioxide
8. References
ASTM A283 / A283M: 2018 Standard Specification for
Low and Intermediate Tensile Strength Carbon Steel
Plates
Standards
ASTM A384
ASTM A36 ASTM A384 / A384M: 2019 Standard Practice for
ASTM A36 / A36M: 2019 Standard Specification for Safeguarding Against Warpage and Distortion During
Carbon Structural Steel Hot­Dip Galvanizing of Steel Assemblies
ASTM A123 ASTM A385
ASTM A123 / A123M: 2017 Standard Specification for ASTM A385 / A385M: 2020 Standard Practice for
Zinc (Hot­Dip Galvanized) Coatings on Iron and Steel Providing High­Quality Zinc Coatings (Hot­Dip)
Products
ASTM A514
ASTM A143 ASTM A514 / A514M: 2018 Standard Specification for
ASTM A143 / A143M: 2020 Standard Practice for High­Yield­Strength, Quenched and Tempered Alloy
Safeguarding Against Embrittlement of Hot­Dip Steel Plate
Galvanized Structural Steel Products and Procedure
for Detecting Embrittlement ASTM A572
ASTM A572 / A572M: 2021 Standard Specification for
ASTM A153 High­Strength Low­Alloy Columbium­Vanadium
ASTM A153 / A153M: 2016 Standard Specification for Structural Steel
Zinc Coating (Hot­Dip) on Iron and Steel Hardware
ASTM A573
ASTM A283 ASTM A573 / A573M: 2020 Standard Specification for
Structural Carbon Steel Plates
10 Environmental Product Declaration ZINQ Technologie GmbH – duroZINQ(R) hot­dip galvanized steel
ASTM A588 EN 14025
ASTM A588 / A588M: 2019 Standard Specification for DIN EN ISO 14025:2010 Environmental labels and
High­Strength Low­Alloy Structural Steel, up to 50 ksi declarations. Type III environmental declarations.
[345 MPa] Minimum Yield Point, with Atmospheric Principles and procedures
Corrosion Resistance
EN ISO 14713-1
ASTM A633 EN ISO 14713­1: 2017 Zinc coatings ­ Guidelines and
ASTM A633 / A633M: 2018 Standard Specification for recommendations for the protection against corrosion
Normalized High­Strength Low­Alloy Structural Steel of iron and steel in structures ­ Part 1: General
Plates principles of design and corrosion resistance
ASTM A709 EN ISO 14713-2
ASTM A709 / A709M: 2018 Standard Specification for EN ISO 14713­2:2020 Zinc coatings ­ Guidelines and
Structural Steel for Bridges recommendations for the protection against corrosion
of iron and steel in structures ­ Part 2: Hot dip
ASTM A913 galvanizing
ASTM A913 / A913M: 2019 Standard Specification for
High­Strength Low­Alloy Steel Shapes of Structural EN 15804
Quality, Produced by Quenching and Self­Tempering EN 15804+A2 Sustainability of construction works ­
Process (QST) Environmental product declarations ­ Core rules for the
product category of construction products
ASTM A992
ASTM A992 / A992M: 2020 Standard Specification for EN 15978
Structural Steel Shapes DIN EN 15978
Sustainability of construction works ­ Assessment of
ASTM A1066 environmental performance of buildings ­ Calculation
ASTM A1066 / A1066M: 2015 Standard Specification method
for High­Strength Low­Alloy Structural Steel Plate
Produced by Thermo­Mechanical Controlled Process ISO 14001
(TMCP) ISO 14001:2015 Environmental management
systems ­ Requirements with guidance for use
DIN EN ISO 12944-2
DIN EN ISO 12944­2 Paints and varnishes ­ Corrosion ISO 45001
protection of steel structures by protective paint ISO 45001: 2018 Occupational health and safety
systems ­ Part 2: Classification of environments management systems ­ Requirements with guidance
for use
EN 1090-1
EN 1090­1:2012 Execution of steel structures and ISO 50001
aluminium structures ­ Part 1: Requirements for ISO 5001:2018 Energy management systems ­
conformity assessment of structural components Requirements with guidance for use
EN 1090-2
EN 1090­2:2018 Execution of steel structures and Further references
aluminium structures ­ Part 2: Technical requirements
for steel structures CPR
Regulation (EU) No 305/2011: Harmonised conditions
EN ISO 1461 for the marketing of construction products, https://eur­
EN ISO 1461:2009 Hot dip galvanized coatings on lex.europa.eu/legal­
fabricated iron and steel articles ­ Specifications and content/EN/TXT/?uri=celex%3A32011R0305
test methods
Cradle-to-Cradle Certification
EN 1993 Guidance for the Cradle to Cradle Certified™ Product
EN 1993 Eurocode 3 ­ Design of steel structures Standard, Cradle to Cradle Products Innovation
Institute www.c2ccertified.com
EN 1994
EN 1994 Eurocode 4: Design of composite steel and EPD of Structural Steel: Sections and Plates
concrete structures Environmental Product Declaration: Structural Steel:
Sections and Plates. bauforumstahl e.V., EPD­BFS­
EN 10025 20180116­IBG2­EN. Berlin: Institut Bauen und Umwelt
EN 10025 Hot rolled products of structural steel e.V. (ed.), 25.10.2018.
EN 10025-1 EWC
EN 10025­1: 2005 Hot rolled products of structural European Waste Catalogue, established by
steels – Part 1: General technical delivery conditions Commission decision 2000/532/EC2
EN 13501 GaBi Database
BS EN 13501­1:2018 Fire classification of construction Sphera Solutions GmbH. (2020). GaBi LCA Database
products and building elements Classification using Documentation. Retrieved from
data from reaction to fire tests gabi.sphera.com/international/support/gabi/
11 Environmental Product Declaration ZINQ Technologie GmbH – duroZINQ(R) hot­dip galvanized steel
GaBi Software PCR Part A
Sphera Solutions GmbH. (2020). GaBi Software. For Calculation Rules for the Life Cycle Assessment and
further information see: Requirements on the Project Report according to EN
gabi.sphera.com/international/index/ 15804+A2:2. Institut Bauen und Umwelt e.V. (IBU).
November 2021. www.ibu­epd.com
German Nutrition Society (DGE)
German Nutrition Society / Deutsche Gesellschaft für PCR Part B
Ernäherung e.V. (DGE), reference values for Nutrient Requirements on the EPD for www.ibu­epd.com
intake, www.dge.de Structural steels. Institut Bauen und Umwelt e.V. (IBU).
November 2021. www.ibu­epd.com
IBU 2021
General Instructions for the EPD programme of Institut
Bauen und Umwelt e.V. Version 2.0, Berlin: Institut
Bauen und Umwelt e.V., 2021. www.ibu­epd.com
12 Environmental Product Declaration ZINQ Technologie GmbH – duroZINQ(R) hot­dip galvanized steel
Publisher
Institut Bauen und Umwelt e.V. Tel +49 (0)30 3087748­ 0
Panoramastr. 1 Fax +49 (0)30 3087748­ 29
10178 Berlin Mail info@ibu­epd.com
Germany Web www.ibu-epd.com
Programme holder
Institut Bauen und Umwelt e.V. Tel +49 (0)30 ­ 3087748­ 0
Panoramastr 1 Fax +49 (0)30 – 3087748 ­ 29
10178 Berlin Mail info@ibu­epd.com
Germany Web www.ibu-epd.com
Author of the Life Cycle
Assessment Tel +49 711 341817­0
Sphera Solutions GmbH Fax +49 711 341817­25
Hauptstraße 111­ 113 Mail info@sphera.com
70771 Leinfelden­Echterdingen Web www.sphera.com
Germany
Tel +49 711 341817­0
Sphera Solutions GmbH Fax +49 711 341817­25
Hauptstr. 111­113 https://sphera.com/
70771 Leinfelden­Echterdingen
Germany Tel +49 209 9403400
Fax +49 209 9403444
ZINQ Technologie GmbH Mail thomas.pinger@zinq.com
An den Schleusen 6 Web www.zinq.com
45881 Gelsenkirchen
Germany
Owner of the Declaration
ZINQ Technologie GmbH Tel +49 209 9403400
An den Schleusen 6 Fax +49 209 9403444
45881 Gelsenkirchen Mail thomas.pinger@zinq.com
Germany Web www.zinq.com
