ENVIRONMENTAL PRODUCT DECLARATION
as per ISO 14025 and EN 15804+A1
Owner of the Declaration Associated Weavers Europe NV
Programme holder Institut Bauen und Umwelt e.V. (IBU)
Publisher Institut Bauen und Umwelt e.V. (IBU)
Declaration number EPD-AWE-20220018-CBA1-EN
Issue date 16.02.2022
Valid to 15.02.2027
Sedna Range
Tufted broadloom carpets with a maximum total pile weight
of 2878 g/m2 and a pile material of 100% regenerated
polyamide 6
Associated Weavers Europe NV
www.ibu-epd.com | https://epd-online.com
Umwelt Produktdeklaration Name des Herstellers – Name des Produkts
General Information
Associated Weavers Europe NV Sedna Range
Tufted broadloom carpet
maximum pile weight of 2878 g/m2
100% regenerated PA6 yarn
Textile polyester backing with 100%
recycled material
Programme holder Owner of the declaration
IBU – Institut Bauen und Umwelt e.V. Associated Weavers Europe NV
Panoramastr. 1 Industriepark Klein Frankrijk
10178 Berlin Weverijstraat 1
Germany 9600 Ronse
Belgium
Declaration number Declared product / declared unit
EPD-AWE-20220018-CBA1-EN Sedna Range - 1 m² tufted broadloom carpet with a
surface pile of 100% regenerated PA 6 and a polyester
Eco FusionBac backing.
This declaration is based on the product Scope:
category rules: The manufacturer declaration applies to broadloom
Floor coverings, 02/2018 carpets with Eco FusioBac, a pile material of PA 6 with
(PCR checked and approved by the SVR) 100% recycled content and a maximum total pile
weight of 2878 g/m2. The products are produced in
Ronse, Belgium.
Issue date
LCA results for products with a maximum total pile
16.02.2022
weight of 800 g/m2 can be taken from the
corresponding tables of the annexe. Specific data for
Valid to
every product within the declared group of products in
15.02.2027 relation to its total pile weight can be calculated by
using equation 1 given in the annexe (see annexe
chapter: 'General Information on the annexe'). The
declaration is only valid in conjunction with a valid
GUT-PRODIS license of the product.
The owner of the declaration shall be liable for the
underlying information and evidence; the IBU shall not
be liable with respect to manufacturer information, life
cycle assessment data and evidences.
The EPD was created according to the specifications
of EN 15804+A1. In the following, the standard will be
simplified as EN 15804.
Verification
The standard EN 15804 serves as the core PCR
Independent verification of the declaration and data
according to ISO 14025:2011
Dipl. Ing. Hans Peters internally x externally
(chairman of Institut Bauen und Umwelt e.V.)
Dr. Alexander Röder Angela Schindler
(Managing Director Institut Bauen und Umwelt e.V.)) (Independent verifier)
Product
Product description/Product definition to 82% with a total pile weight of 2878 g/m2. The
Tufted broadloom carpets having a surface pile of declaration applies to a group of products with a
100% regenerated polyamide 6 and an Eco FusionBac maximum total pile weight of 2878 g/m2. LCA results
backing. The colour of the carpet is generated by for products with a maximum total pile weight of 800
continuous dyeing. The total recycled content amounts g/m2 can be taken from the corresponding tables of the
2 Environmental Product Declaration Associated Weavers Europe NV (AW) – Sedna Range - Tufted Broadloom carpet with
100% recycled PA6 yarn
annexe. Results for specific products with any other
total pile weight can be calculated by using equation 1 Base materials/Ancillary materials
given in the annexe (see annexe chapter: 'General
Information on the annexe'). Name Value Unit
Polyamide 6 79,3 %
For the placing on the market of the product in the Polyester 2,7 %
European Union/European Free Trade Association SBR-latex 3,6 %
(EU/EFTA) (with the exception of Switzerland) Polypropylene 2,7 %
Regulation (EU) No. 305/2011 Construction Product Limestone 11,7 %
Regulation (CPR) applies. The product needs a Additives 0,01 %
Declaration of Performance (DoP) taking into This product contains substances listed in the ECHA
consideration EN 14041: 2018-05, Resilient, textile and candidate list (16.01.2020) or other carcinogenic,
laminate floor coverings - Essential characteristics, and mutagenic or reprotoxic (CMR) substances in
the CE-marking. The DoP of the product can be found categories 1A or 1B which are not on the candidate list
on the manufacturer's technical information section. exceeding 0.1 percentage by mass: no.
For the application and use of the product the The products are registered in the GUT-PRODIS
respective national provisions apply. Information System. The PRODIS system ensures the
compliance with limitations of various chemicals and
Application Volatile Organic Compound (VOC)-emissions and a
According to the use class as defined in EN 1307 the ban on the use of all substances that are listed as
products can be used in all professional areas. The 'Substances of Very High Concern' (SVHC) under
use class can be found on the technical data sheet of REACH.
the product.
Reference service life
Technical Data A calculation of the reference service life according to
ISO 15686 is not possible.
The service life of textile floor coverings strongly
depends on the correct installation taking into account
Name Value Unit the declared use classification and the adherence to
Product Form broadloom carpets -
cleaning and maintenance instructions.
Type of manufacture Tufted carpets - A minimum service life of 10 years can be
Yarn type Polyamide 6 - assumed, technical service life can be considerably
Coloration continuous dyed surface longer.
Primary backing Polypropylene
Secondary backing Polyester -
Total pile weight max. 2878 g/m²
Total carpet weight max. 3630 g/m2
Performance data of the product in accordance with
the declaration of performance with respect to its
essential characteristics according to EN 14041: 2018-
05, Resilient, textile and laminate floor coverings -
Essential characteristics. Additional product properties
in accordance with EN 1307 can be found on the
Product Information System PRODIS using the
PRODIS registration number of the product (www.pro-
dis.info) or on the manufacturer's technical information
section (www.carpetyourlife.com).
LCA: Calculation rules
Declared Unit Modules C3, C4 and D are indicated separately for
three end-of-life scenarios:
1 - landfill disposal
Name Value Unit 2 - municipal waste incineration
Declared unit 1 m2 3 - recovery in a cement plant
Conversion factor to 1 kg 3.63 -
The declared unit refers to 1 m2 produced textile floor
covering. The output of module A5 'Assembly' is 1 m2
installed textile floor covering. A1-A3 Production:
Energy supply and production of the basic material,
processing of secondary material, auxiliary material,
System boundary transport of the material to the manufacturing site,
emissions, waste water treatment, packaging material
Type of EPD: Cradle-to-grave and waste processing up to the landfill disposal of
residual waste (except radioactive waste). Benefits for
System boundaries of modules A, B, C, D: generated electricity and steam due to the incineration
of production waste are aggregated.
3 Environmental Product Declaration Associated Weavers Europe NV (AW) – Sedna Range - Tufted Broadloom carpet with
100% recycled PA6 yarn
Biogenic carbon that is stored in renewable material
(packaging paper) is taken into account as well as the C2 Transport:
associated carbon dioxide uptake from the air from Transport of the carpet waste to a landfill, to the
which this biogenic carbon comes. municipal waste incineration plant (MWI) or to the
waste collection facility for recycling.
A4 Transport:
Transport of the packed textile floor covering C3 Waste processing:
from factory gate to the place of installation. C3-1: Landfill disposal needs no waste processing.
C3-2: Impact from waste incineration (plant with
A5 Installation: R1>0.6), generated electricity and steam are listed in
Installation of the textile floor covering, processing of the result table as exported energy.
installation waste and packaging waste up to the C3-3: Collection of the carpet waste for recovery in the
landfill disposal of residual waste (except radioactive cement industry, waste processing (granulating),
waste), the production of the amount of carpet that transport to the cement plant, emissions from the
occurs as installation waste including its transport to incineration. The biogenic carbon that is stored in the
the place of installation. renewable materials of the floor covering is released
Generated electricity and steam due to the incineration into the air as carbon dioxide emissions.
of waste are listed in the result table as exported
energy. C4 Disposal
Biogenic carbon that is stored in renewable materials C4-1: Impact from landfill disposal,
in packaging paper is released as carbon dioxide C4-2: The carpet waste leaves the system in
emissions into the air at the end of life in module A5. module C3-2,
Preparation of the floor and auxiliary materials C4-3: The pre-processed carpet waste leaves the
(adhesives, fixing agents, PET connectors) are beyond system in module C3-3.
the system boundaries and not taken into account.
D Recycling potential:
B1 Use: Calculated benefits result from materials exclusive
Indoor emissions during the use stage. After the first secondary materials (net materials).
year, no product-related Volatile Organic Compound D-A5: Benefits for generated energy due
(VOC) emissions are relevant due to known VOC to incineration of packaging and installation waste
decay curves of the product. (incineration plant with R1 > 0.6),
D-1: Benefits for generated energy due to landfill
B2 Maintenance: disposal of carpet waste at the end-of-life,
Cleaning of the textile floor covering for a period of 1 D-2: Benefits for generated energy due to incineration
year: of carpet waste at the end-of-life (incineration plant
Vacuum cleaning – electricity supply with R1 > 0.6),
Wet cleaning – electricity, water consumption, D-3: Benefits for saved fossil energy and saved
production of the cleaning agent, waste water inorganic material due to recovery of the carpet in a
treatment. cement plant.
The declared values in this module have to be
multiplied by the assumed service life of the floor Comparability
covering in the building in question. Basically, a comparison or an evaluation of EPD data
is only possible if all the data sets to be compared
B3 - B7: were created according to EN 15804 and the building
The modules are not relevant and therefore not context, respectively the product-specific
declared. characteristics of performance, are taken into account.
C1 De-construction: Background data are taken from the GaBi database
The floor covering is de-constructed manually and no 2021. Remaining data gaps are covered by the
additional environmental impact is caused. ecoinvent 3.7 database
LCA: Scenarios and additional technical information
The following information refer to the declared modules Preparation of the floor and auxiliaries (adhesives,
and are the basis for calculations or can be used for fixing agents, PET connectors etc.) are not taken into
further calculations. account.
Transport to the construction site (A4) Maintenance (B2)
Name Value Unit The values for cleaning refer to 1 m2 floor covering
Litres of fuel (truck, EURO 0-6 mix) 0.0085 l/100km used in commercial areas per year. Depending on the
Transport distance 700 km application based on ISO 10874, the technical service
Capacity utilisation (including empty life recommended by the manufacturer and the
55 %
runs) anticipated strain on the floor by customers, the case-
specific useful life can be established. Based on this
Installation in the building (A5) useful life the effects of Module B2 need to be
Name Value Unit calculated in order to obtain the overall environmental
Material loss 0.33 kg impacts.
Polyethylene packaging waste and installation waste Name Value Unit
are considered to be incinerated in a municipal waste Maintenance cycle (wet cleaning) 1.5 1/year
incineration plant. Cardboard is going to be recycled. Maintenance cycle (vacuum cleaning) 208 1/year
4 Environmental Product Declaration Associated Weavers Europe NV (AW) – Sedna Range - Tufted Broadloom carpet with
100% recycled PA6 yarn
Water consumption (wet cleaning) 0.004 m3
Cleaning agent (wet cleaning) 0.09 kg
Electricity consumption 0.314 kWh
Further information on cleaning and maintenance see
www.carpetyourlife.com
End of Life (C1-C4)
Three different end-of-life scenarios are declared and
the results are indicated separately in module C.
Each scenario is calculated as a 100 % scenario.
Scenario 1: 100 % landfill disposal
Scenario 2: 100 % municipal waste incineration (MWI)
with R1>0.6
Scenario 3: 100 % recycling in the cement industry
If combinations of these scenarios have to be
calculated this should be done according to the
following scheme:
EOL-impact = x % impact (Scenario 1)
+ y % impact (Scenario 2)
+ z % impact (Scenario 3)
with x % + y % + z % = 100%
Name Value Unit
Collected as mixed construction
3.63 kg
waste (scenario 1 and 2)
Collected separately (scenario 3) 3.63 kg
Landfilling (scenario 1) 3.63 kg
Energy recovery (scenario 2) 3.63 kg
Energy recovery (scenario 3) 3,204 kg
Recycling (scenario 3) 0.426 kg
Reuse, recovery and/or recycling potentials (D),
relevant scenario information
Recovery or recycling potentials due to the three end-
of-life scenarios (module C) are indicated separately.
Recycling in the cement industry (scenario 3)
VDZ e.V.
The organic material of the carpet is used as
secondary fuel in a cement kiln. It mainly substitutes
for lignite (65.5 %), hard coal (26.2 %) and petrol coke
(8.6 %).
The inorganic material is substantially integrated into
the cement clinker and substitutes for original material
input.
5 Environmental Product Declaration Associated Weavers Europe NV (AW) – Sedna Range - Tufted Broadloom carpet with
100% recycled PA6 yarn
LCA: Results
The LCA results refer to all declared products with a maximum total pile weight of 2878 g/m2. LCA results for
products with a maximum total pile weight of 800 g/m2 can be taken from the corresponding tables of the annexe.
Results for specific products with any other total pile weight can be calculated by using equation 1 given in the
annexe (see annexe chapter: 'General Information on the annexe'). The declared result figures in module B2 have
to be multiplied by the assumed service life (in years) of the floor covering in the building under consideration.
Information on non-relevant modules: Modules B3 - B7 are not relevant during the service life of the carpet.
Modules C1, C3/1, C4/2 and C4/3 cause no additional impact (see chapter "LCA: Calculation rules" in this
document). All these modules are declared and marked as 'modules not relevant/declared'. Module C2 represents
the transport for scenarios 1, 2 and 3. Column D represents module D/A5. The calculations are based on the CML
characterization factors (version August 2016).
DESCRIPTION OF THE SYSTEM BOUNDARY (X = INCLUDED IN LCA; MND = MODULE NOT DECLARED;
MNR = MODULE NOT RELEVANT)
BENEFITS AND
CONSTRUCTI LOADS
PRODUCT STAGE ON PROCESS USE STAGE END OF LIFE STAGE BEYOND THE
STAGE SYSTEM
BOUNDARIES
6 Environmental Product Declaration Associated Weavers Europe NV (AW) – Sedna Range - Tufted Broadloom carpet with
100% recycled PA6 yarn
lairetam
waR
ylppus tropsnarT
gnirutcafunaM
eht
morf
tropsnarT
etis
eht
ot
etag
ylbmessA esU
ecnanetniaM
riapeR
tnemecalpeR tnemhsibrufeR
ygrene
lanoitarepO esu
retaw
lanoitarepO esu
noitcurtsnoc-eD
noitilomed tropsnarT
gnissecorp
etsaW
lasopsiD -esueR -yrevoceR -gnilcyceR laitnetop
A1 A2 A3 A4 A5 B1 B2 B3 B4 B5 B6 B7 C1 C2 C3 C4 D
X X X X X X X MNR MNR MNR MND MND MND X X X X
RESULTS OF THE LCA - ENVIRONMENTAL IMPACT according to EN 15804+A1: 1 m² floorcovering
Parameter Unit A1-A3 A4 A5 B1 B2 C2 C3/2 C3/3 C4/1 D D/1 D/2 D/3
GWP [kg CO2-Eq.] 7.10E+0 2.13E-1 1.37E+0 0.00E+0 1.71E-1 1.20E-2 7.48E+0 7.57E+0 2.47E-1 -2.35E-2 0.00E+0 -1.67E-1 -4.30E-2
-3.57E- -2.49E- -1.88E-
ODP [kg CFC11-Eq.] 3.36E-8 3.71E-17 3.02E-9 0.00E+0 2.37E-9 2.10E-181.86E-152.51E-158.37E-16 0.00E+0
16 15 16
AP [kg SO2-Eq.] 2.96E-2 8.79E-4 3.47E-3 0.00E+0 4.46E-4 4.98E-5 8.00E-3 8.16E-3 6.40E-4 -2.71E-5 0.00E+0 -1.91E-4 -1.17E-4
EP [kg (PO4)3--Eq.] 6.62E-3 2.24E-4 8.06E-4 0.00E+0 9.11E-5 1.27E-5 2.09E-3 2.13E-3 6.94E-4 -3.73E-6 0.00E+0 -2.63E-5 -1.93E-5
POCP [kg ethene-Eq.] 2.09E-3 -3.77E-4 1.95E-4 6.29E-5 4.69E-5 -2.13E-5 4.75E-4 4.25E-4 5.76E-5 -2.49E-6 0.00E+0 -1.76E-5 -1.58E-5
ADPE [kg Sb-Eq.] 7.94E-6 1.88E-8 7.25E-7 0.00E+0 6.39E-7 1.07E-9 9.73E-8 1.07E-7 4.73E-8 -4.39E-9 0.00E+0 -3.08E-8 -4.84E-9
ADPF [MJ] 9.79E+1 2.89E+0 9.41E+0 0.00E+0 2.68E+0 1.64E-1 3.59E+0 4.22E+0 3.68E+0 -3.39E-1 0.00E+0-2.41E+0-6.24E+0
GWP = Global warming potential; ODP = Depletion potential of the stratospheric ozone layer; AP = Acidification potential of land and water; EP =
Caption Eutrophication potential; POCP = Formation potential of tropospheric ozone photochemical oxidants; ADPE = Abiotic depletion potential for non-
fossil resources; ADPF = Abiotic depletion potential for fossil resources
RESULTS OF THE LCA - INDICATORS TO DESCRIBE RESOURCE USE according to EN 15804+A1: 1 m²
floorcovering
Parameter Unit A1-A3 A4 A5 B1 B2 C2 C3/2 C3/3 C4/1 D D/1 D/2 D/3
PERE [MJ] 1.23E+2 1.62E-1 1.12E+1 0.00E+0 1.15E+0 9.17E-3 4.14E-1 6.02E-1 2.75E-1 -9.20E-2 0.00E+0 -6.43E-1 -4.64E-2
PERM [MJ] 7.30E-2 0.00E+0 -7.30E-2 0.00E+0 0.00E+0 0.00E+0 0.00E+0 0.00E+0 0.00E+0 0.00E+0 0.00E+0 0.00E+0 0.00E+0
PERT [MJ] 1.23E+2 1.62E-1 1.11E+1 0.00E+0 1.15E+0 9.17E-3 4.14E-1 6.02E-1 2.75E-1 -9.20E-2 0.00E+0 -6.43E-1 -4.64E-2
PENRE [MJ] 9.64E+1 2.90E+0 1.02E+1 0.00E+0 3.64E+0 1.65E-1 1.08E+1 1.16E+1 3.79E+0 -4.13E-1 0.00E+0 -2.93E+0 -6.26E+0
PENRM [MJ] 7.21E+0 0.00E+0 -2.41E-1 0.00E+0 0.00E+0 0.00E+0 -6.97E+0 -6.97E+0 0.00E+0 0.00E+0 0.00E+0 0.00E+0 0.00E+0
PENRT [MJ] 1.04E+2 2.90E+0 9.95E+0 0.00E+0 3.64E+0 1.65E-1 3.83E+0 4.60E+0 3.79E+0 -4.13E-1 0.00E+0 -2.93E+0 -6.26E+0
SM [kg] 3.10E+0 0.00E+0 2.79E-1 0.00E+0 0.00E+0 0.00E+0 0.00E+0 0.00E+0 0.00E+0 0.00E+0 0.00E+0 0.00E+0 2.40E-1
RSF [MJ] 0.00E+0 0.00E+0 0.00E+0 0.00E+0 0.00E+0 0.00E+0 0.00E+0 0.00E+0 0.00E+0 0.00E+0 0.00E+0 0.00E+0 0.00E+0
NRSF [MJ] 0.00E+0 0.00E+0 0.00E+0 0.00E+0 0.00E+0 0.00E+0 0.00E+0 0.00E+0 0.00E+0 0.00E+0 0.00E+0 0.00E+0 0.00E+0
FW [m³] 3.53E-1 1.85E-4 3.35E-2 0.00E+0 1.77E-3 1.05E-5 1.90E-2 1.92E-2 3.50E-5 -8.98E-5 0.00E+0 -6.28E-4 -5.09E-4
PERE = Use of renewable primary energy excluding renewable primary energy resources used as raw materials; PERM = Use of
renewable primary energy resources used as raw materials; PERT = Total use of renewable primary energy resources; PENRE = Use of
non-renewable primary energy excluding non-renewable primary energy resources used as raw materials; PENRM = Use of non-
Caption
renewable primary energy resources used as raw materials; PENRT = Total use of non-renewable primary energy resources; SM = Use
of secondary material; RSF = Use of renewable secondary fuels; NRSF = Use of non-renewable secondary fuels; FW = Use of net fresh
water
RESULTS OF THE LCA – WASTE CATEGORIES AND OUTPUT FLOWS according to EN 15804+A1:
1 m² floorcovering
Parameter Unit A1-A3 A4 A5 B1 B2 C2 C3/2 C3/3 C4/1 D D/1 D/2 D/3
HWD [kg] 8.19E-3 1.46E-10 7.37E-4 0.00E+0 6.35E-10 8.29E-12 9.31E-10 1.05E-9 6.82E-10 -9.26E-11 0.00E+0 -6.55E-10-3.98E-11
NHWD [kg] 1.12E+0 4.31E-4 1.24E-1 0.00E+0 2.59E-3 2.44E-5 2.49E-1 2.50E-1 3.62E+0 -1.92E-4 0.00E+0 -1.36E-3 -1.55E-4
RWD [kg] 2.06E-3 3.51E-6 1.94E-4 0.00E+0 3.57E-4 1.99E-7 9.55E-5 1.49E-4 4.40E-5 -2.96E-5 0.00E+0 -2.07E-4 -1.03E-5
CRU [kg] 0.00E+0 0.00E+0 0.00E+0 0.00E+0 0.00E+0 0.00E+0 0.00E+0 0.00E+0 0.00E+0 0.00E+0 0.00E+0 0.00E+0 0.00E+0
MFR [kg] 2.12E-2 0.00E+0 2.45E-2 0.00E+0 0.00E+0 0.00E+0 0.00E+0 2.40E-1 0.00E+0 0.00E+0 0.00E+0 0.00E+0 0.00E+0
MER [kg] 0.00E+0 0.00E+0 0.00E+0 0.00E+0 0.00E+0 0.00E+0 0.00E+0 0.00E+0 0.00E+0 0.00E+0 0.00E+0 0.00E+0 0.00E+0
EEE [MJ] 0.00E+0 0.00E+0 1.35E+0 0.00E+0 0.00E+0 0.00E+0 1.45E+1 0.00E+0 0.00E+0 0.00E+0 0.00E+0 0.00E+0 0.00E+0
EET [MJ] 0.00E+0 0.00E+0 2.41E+0 0.00E+0 0.00E+0 0.00E+0 2.61E+1 0.00E+0 0.00E+0 0.00E+0 0.00E+0 0.00E+0 0.00E+0
HWD = Hazardous waste disposed; NHWD = Non-hazardous waste disposed; RWD = Radioactive waste disposed; CRU = Components
Caption for re-use; MFR = Materials for recycling; MER = Materials for energy recovery; EEE = Exported electrical energy; EEE = Exported
thermal energy
References
EN 1307 CML characterization factors
DIN EN 1307: 2014+A1:2016+A2:2018-05: Textile Impact assessment characterization factors, version
floor coverings - Classification 4.7, August 2016, Institute of Environmental Sciences -
'Centrum voor Milieuwetenschappen in Leiden' (CML),
EN 13501-1 Leiden, The Netherlands
DIN EN 13501-1:2019-05: Fire classification of
construction products and building elements - Part 1:
Classification using data from reaction to fire tests ECHA candidate list
Candidate List of substances of very high concern
EN 14041 (SVHCs) for authorisation, 16.01.2020, European
DIN EN 14041: 2018-05: Resilient, textile and laminate Chemicals Agency (ECHA), Helsinki, Finland
floor coverings - Essential characteristics
ecoinvent 3.7
EN 15804 ecoinvent, Zurich, Switzerland, database version 3.7,
EN 15804:2012-04+A1 2013/, Sustainability of published September 2020
construction works — Environmental Product
Declarations — Core rules for the product category of GaBi database 2021
construction products GaBi Software-System and Database for Life Cycle
Engineering, thinkstep AG, Leinfelden-Echterdingen,
EN 16810 Database release 2021-2
DIN EN 16810: 2017-08: Resilient, textile and laminate
floor coverings – Environmental product declarations – IBU 2021
Product category rules IBU (2021): General Programme Instructions for the
Preparation of EPDs at the Institut Bauen und Umwelt
ISO 10874 e.V., Version 2.0 Institut Bauen und Umwelt e.V.,
DIN EN ISO 10874: 2012+A1:2021-04: Resilient, Berlin. www.ibu-epd.de
textile and laminate floor coverings - Classification
PCR Part A
ISO 14025 Product Category Rules for Construction Products
DIN EN /ISO 14025:2011-10/, Environmental labels from the range of Environmental Product Declarations.
and declarations — Type III environmental Part A: Calculation Rules for the Life Cycle
declarations — Principles and procedures Assessment and Requirements on the Background
Report, V1.9, Berlin: Institut Bauen und Umwelt e.V.
ISO 14040 (IBU), January 2021
DIN EN ISO 14040:2006+A1:2020 Environmental
management - Life cycle assessment - Principles and PCR Part B
framework Product Category Rules for Construction Products
from the range of Environmental Product Declarations
ISO 14044 of Institut Bauen und Umwelt (IBU),
DIN EN ISO 14044:2006+A1:2018+A2:2020 Part B: Requirements on the EPD for floor coverings,
Environmental management - Life cycle assessment - V1.2, Berlin: Institut Bauen und Umwelt e.V. (IBU),
Requirements and guidelines February 2018
ISO 15686 PRODIS
ISO 15686: Buildings and constructed assets - Product Information System (PRODIS) of the
Service life planning European Carpet Industry, Gemeinschaft
ISO 15686-1: 2011-05: Part 1: General principles and umweltfreundlicher Teppichboden e.V (GUT) and
framework European Carpet and Rug Association
ISO 15686-2: 2012-05: Part 2: Service life prediction (ECRA), http://www.pro-dis.info
procedures
ISO 15686-7: 2017-04: Part 7: Performance REACH
evaluation for feedback of service life data Regulation (EC) No 1907/2006 of the European
from practice Parliament and of the Council of 18 December 2006
ISO 15686-8: 2008-06: Part 8: Reference service life concerning the Registration, Evaluation, Authorisation
and service-life estimation and Restriction of Chemicals (REACH). Last update:
27.02.2020 (Status: 27.06.2018)
Regulation (EU) No. 305/2011
Regulation No. 305/2011 Construction Products VDZ e.V.
Regulation (CPR) of the European Council and of the Association of German Cement Works, Ed.
European Parliament, April 2011 Environmental Data of the German Cement Industry
2019
7 Environmental Product Declaration Associated Weavers Europe NV (AW) – Sedna Range - Tufted Broadloom carpet with
100% recycled PA6 yarn
Publisher
Institut Bauen und Umwelt e.V. Tel +49 (0)30 3087748- 0
Panoramastr. 1 Fax +49 (0)30 3087748- 29
10178 Berlin Mail info@ibu-epd.com
Germany Web www.ibu-epd.com
Programme holder
Institut Bauen und Umwelt e.V. Tel +49 (0)30 - 3087748- 0
Panoramastr 1 Fax +49 (0)30 – 3087748 - 29
10178 Berlin Mail info@ibu-epd.com
Germany Web www.ibu-epd.com
Author of the Life Cycle
Assessment Tel +49 (0)241 96843 410
Gemeinschaft umweltfreundlicher Fax +49 (0)241 96843 400
Teppichboden (GUT) e.V. Mail mail@gut-ev.de
Schönebergstraße 2 Web www.gut-ev.org
52068 Aachen
Germany
Owner of the Declaration
Associated Weavers Europe NV Tel +32 (0) 55 23 02 11
Weverijstraat 1 Fax -
9600 Ronse Mail info@awe.be
Belgium Web www.carpetyourlife.com
