ENVIRONMENTAL PRODUCT DECLARATION
as per ISO 14025 and EN 15804+A2
Owner of the Declaration KONE Corporation
Publisher Institut Bauen und Umwelt e.V. (IBU)
Programme holder Institut Bauen und Umwelt e.V. (IBU)
Declaration number EPD-KON-20230582-CBA2-EN
Issue date 22.12.2023
Valid to 13.04.2028
UniSwing Compact / Robust / Fire
KONE
www.ibu-epd.com | https://epd-online.com
General Information
KONE UniSwing Compact / Robust / Fire
Programme holder Owner of the declaration
IBU – Institut Bauen und Umwelt e.V. KONE Corporation
Hegelplatz 1 Keilasatama 3
10117 Berlin 02150 ESPOO
Germany Finland
Declaration number Declared product / declared unit
EPD-KON-20230582-CBA2-EN 1 piece of the product: Automatic Swing Door Operator UniSwing
Compact, consisting of the following items:
• UniSwing Compact door operator
• UniSwing Compact slide channel set
• Uni Swing Compact basic cover
• Product packaging
This declaration is based on the product category rules: Scope:
Drive systems for automatic doors and gates, 01.08.2021 This Environmental Product Declaration refers to a specific UniSwing
(PCR checked and approved by the SVR) Compact automatic swing door operator. This EPD is also representative
for the UniSwing Robust and Fire. The production site is located in
Germany. Green electricity is being used at the production site.
Issue date
Data represents the year 2022.
22.12.2023
The owner of the declaration shall be liable for the underlying information
and evidence; the IBU shall not be liable with respect to manufacturer
Valid to
information, life cycle assessment data and evidences.
13.04.2028
The EPD was created according to the specifications of EN 15804+A2. In
the following, the standard will be simplified as EN 15804.
Verification
The standard EN 15804 serves as the core PCR
Independent verification of the declaration and data according to ISO
14025:2011
internally X externally
Dipl.-Ing. Hans Peters
(Chairman of Institut Bauen und Umwelt e.V.)
Florian Pronold Dr.-Ing. Wolfram Trinius,
(Managing Director Institut Bauen und Umwelt e.V.) (Independent verifier)
1 Environmental Product Declaration - KONE - UniSwing Compact / Robust / Fire
Product
The KONE swing door operators have the following technical
Product description/Product definition properties:
The automatic swing door operators are designed for single- or
Name Value Unit
double leaf doors. Depending on the width and weight of the
Height 240 mm
door leaf, the UniSwing Compact, Robust or Fire is required.
The operators can be mounted with standard arm as push- Installation depth 152 mm
version and with slide channel as pull-version. Apart from the Maximum door weight ED 100 272 kg
extended cover, an integrated door coordinator is also available Opening speed maximum 50 cm/s
for double-leaf operators, which is also easily fitted. By using
Closing speed maximum 40 cm/s
the upgrade card, the functional scope can be adapted to a
Hold open time maximum 60 s
variety of door situations.
Supply voltage, frequency maximum 60 Hz
Features Power consumption 175 W
• Flexible configuration of the functions actually required Class of protection 20 IP
• Inexpensive transport and easy assembly thanks to Performance data of the product with respect to its
lower weights characteristics in accordance with the relevant technical
• Low-noise application thanks to multi-stage gear provision which can be applied are mentioned above.
• Elegant design: dormakaba Contur Design with an
operator height of only 70 mm Base materials/Ancillary materials
The major material composition including the packaging of the
For the use and application of the product the respective product is listed below.
national provisions at the place of use apply.
Name Value Unit
• ISO 13849-1 Steel 33 %
• DIN 18650-1
Aluminium 19 %
• DIN 18650-2
Paper 14 %
• EN 16005
• EN 60335-1 Zinc 14 %
• 2011/65/EU ROHS3 Directive Plastic 10 %
• Machinery Directive 2006/42/EC Electronics 9 %
The CE-marking takes into account the proof of conformity with
Brass 1 %
the respective harmonized standards based on the legal
provisions above. The KONE swing door operators include partial articles which
contain substances listed in the Candidate List of REACH
Application Regulation 1907/2006/EC (date: 17.01.2023) exceeding 0.1
KONE swing door operators are suitable for various percentage by mass: yes
applications: • Lead (Pb): 7439-92-1 (CAS-No) is used in the steel
• For single- or double- leaf swing doors alloy. The concentration of lead in the alloy does not
• Assembly on smoke or fire doors: as pull- version with exceed 0,35% (by mass).
slide channels and as push- version with standard arm The Candidate List can be found on the ECHA website
• Automation of doors with low traffic capacity (Low- address: https:echa.europa.eu/de/home.
Energy Mode) and heavily frequented doors (Full-
Reference service life
Energy Mode)
• High torque for full-automatic swing doors with radar The reference service life of the UniSwing Compact, Robust
detector control and Fire amounts to 10 years and depends on the application
• Suitable for internal and external doors and frequency of use. Regular maintenance is advised to
ensure the life expectancy of 10 years. For repairs or renewals,
Technical Data suitable spare parts are available. The swing door operators
are tested and certified to EN 16005, meaning they are
designed to withstand a minium of 1.000.000 cycles.
LCA: Calculation rules
Production - Module A1-A3
Declared Unit The product stage includes:
— A1, raw material extraction, processing and mechanical
The declared unit is 1 piece of the product: UniSwing Compact treatments, processing of secondary material input (e.g.
Name Value Unit recycling processes),
— A2, transport to the manufacturer,
Declared unit 1 pce.
— A3, manufacturing and assembly including provision of all
Mass reference 13.54 kg/pce
materials, products and energy, as well as waste processing up
to the end-of waste state.
System boundary
The type of EPD is: cradle to gate with options, modules C1– Construction stage - Modules A4-A5
C4, and module D (A1–A3 + C + D and additional modules: A4 The construction process stage includes:
+ A5 + B6) — A4, transport to the building site;
— A5, installation into the building; including provision of all
2 Environmental Product Declaration - KONE - UniSwing Compact / Robust / Fire
materials, products and energy, as well as waste processing up includes:
to the end-of waste state or disposal of final residues during the — D, recycling potentials, expressed as net impacts and
construction process stage. benefits.
Use stage - Module B6 Geographic Representativeness
The use stage related to the operation of the building Land or region, in which the declared product system is
includes: manufactured, used or handled at the end of the product´s
— B6, operational energy use lifespan: Global
End-of-life stage– Modules C1-C4 and D
Comparability
The end-of-life stage includes:
Basically, a comparison or an evaluation of EPD data is only
— C1, de-construction, demolition:
possible if all the data sets to be compared were created
— C2, transport to waste processing;
according to EN 15804 and the building context, respectively
— C3, waste processing for reuse, recovery and/or recycling;
the product-specific characteristics of performance, are taken
— C4, disposal; including provision and all transport, provision
into account. Background database: GaBi, SP40
of all materials, products and related energy and water use.
Module D (Benefits and loads beyond the system boundary)
LCA: Scenarios and additional technical information
End of life (C1-C4)
Characteristic product properties of biogenic carbon
C1: The product dismantling from the building is done manually
Name ValueUnit
without environmental burden.
kg
Biogenic carbon content in product 0.27 Name Value Unit
C
Collected separately waste type 12.43 kg
Biogenic carbon content in accompanying kg
packaging 0.41 C Recycling 8.18 kg
Energy recovery 1.89 kg
Note: 1 kg of biogenic carbon is equivalent to 44/12 kg of CO .
2
Landfilling 2.36 kg
Transport to waste management 50 km
The product is disassembled in a recycling process.
Material recycling is then assumed for the metals and
Transport from the gate to the site (A4) electronics. The plastic components are assumed to be
incinerated with energy recovery. Electromechanics and minor
Name Value Unit
proportions of residues arising from the recycling process are
Litres of fuel (per 1 kg) 0.00276 l/100km
landfilled.
Capacity utilisation (including empty runs) 55 % Region for the End of Life is: Global.
Transport distance via medium truck 100 km
The product is transported via truck. Reuse, recovery and/or recycling potentials (D), relevant
scenario information
Installation into the building (A5) Name Value Unit
Name Value Unit Recycling 100 %
Waste packaging (paper and plastic) 1,11 kg Collection rate is 100%.
Reference service life
Name Value Unit
Life Span according to the manufacturer 10 a
Operational energy use (B6)
Name ValueUnit
Electricity consumption UniSwing Compact for 1
70.42 kWh
year
Days per year in use 365 days
On mode per day 1.8 h
Idle mode per day 22.2 h
On mode power 22.09 W
Idle mode power 6.9 W
3 Environmental Product Declaration - KONE - UniSwing Compact / Robust / Fire
LCA: Results
DESCRIPTION OF THE SYSTEM BOUNDARY (X = INCLUDED IN LCA; MND = MODULE OR INDICATOR NOT DECLARED; MNR
= MODULE NOT RELEVANT)
Benefits and
Construction loads beyond
Product stage Use stage End of life stage
process stage the system
boundaries
la ire ta m w a Ry lp p u s tro p s n a rT g n iru tc a fu n a M e h t m o rf tro p s n a rTe tis e h t o t e ta g y lb m e s s A e s U e c n a n e tn ia M ria p e R tn e m e c a lp e R tn e m h s ib ru fe R y g re n e la n o ita re p Oe s u re ta w la n o ita re p Oe s u n o itc u rts n o c -e Dn o itilo m e d tro p s n a rT g n is s e c o rp e ts a W la s o p s iD -e s u e R-y re v o c e R-g n ilc y c e Rla itn e to p
A1 A2 A3 A4 A5 B1 B2 B3 B4 B5 B6 B7 C1 C2 C3 C4 D
X X X X X MND MND MNR MNR MNR X MND X X X X X
RESULTS OF THE LCA - ENVIRONMENTAL IMPACT according to EN 15804+A2: 1 piece UniSwing Compact / Robust / Fire
Parameter Unit A1-A3 A4 A5 B6 C1 C2 C3 C4 D
GWP-total kg CO 2 eq 5.01E+01 1.18E-01 1.57E+00 2.85E+02 0 6.2E-02 6.22E+00 4.2E-02 -1.39E+01
GWP-fossil kg CO 2 eq 5.27E+01 1.13E-01 3.9E-02 2.83E+02 0 5.9E-02 4.89E+00 4.2E-02 -1.38E+01
GWP-biogenic kg CO 2 eq -2.72E+00 5E-03 1.53E+00 9.45E-01 0 3E-03 1.33E+00 1.43E-04 -3.6E-02
GWP-luluc kg CO 2 eq 6.7E-02 2.69E-06 2.58E-05 4.11E-01 0 1.4E-06 2.88E-04 1.21E-04 -7E-03
ODP kg CFC11 eq 4.49E-09 1.2E-17 2.83E-16 6.24E-12 0 6.22E-18 2.62E-15 1.55E-16 -2.62E-11
AP mol H+ eq 2.14E-01 1.13E-04 4.39E-04 6.26E-01 0 5.89E-05 1E-03 3.01E-04 -5.3E-02
EP-freshwater kg P eq 2.04E-04 2.42E-08 5.53E-08 7.57E-04 0 1.26E-08 4.16E-07 7.2E-08 -2.37E-05
EP-marine kg N eq 3.8E-02 3.61E-05 1.59E-04 1.39E-01 0 1.88E-05 2.58E-04 7.74E-05 -7E-03
EP-terrestrial mol N eq 4E-01 4.01E-04 2E-03 1.46E+00 0 2.09E-04 5E-03 8.5E-04 -7.9E-02
kg NMVOC
POCP 1.19E-01 1.02E-04 4.2E-04 3.81E-01 0 5.3E-05 7.12E-04 2.34E-04 -2.6E-02
eq
ADPE kg Sb eq 1.12E-02 3.4E-09 4.46E-09 8.21E-05 0 1.77E-09 3.63E-08 3.76E-09 -3E-03
ADPF MJ 8.17E+02 1.61E+00 4.95E-01 4.98E+03 0 8.35E-01 2.55E+00 5.5E-01 -1.9E+02
m3 world eq
WDP 9.42E+00 2.22E-04 1.94E-01 6.18E+01 0 1.15E-04 6.37E-01 4E-03 -1.88E+00
deprived
GWP = Global warming potential; ODP = Depletion potential of the stratospheric ozone layer; AP = Acidification potential of land and water; EP =
Eutrophication potential; POCP = Formation potential of tropospheric ozone photochemical oxidants; ADPE = Abiotic depletion potential for non-fossil
resources; ADPF = Abiotic depletion potential for fossil resources; WDP = Water (user) deprivation potential)
RESULTS OF THE LCA - INDICATORS TO DESCRIBE RESOURCE USE according to EN 15804+A2: 1 piece UniSwing Compact
/ Robust / Fire
Parameter Unit A1-A3 A4 A5 B6 C1 C2 C3 C4 D
PERE MJ 1.92E+02 5E-03 1.34E+01 2.21E+03 0 3E-03 9.52E+00 7.2E-02 -4.87E+01
PERM MJ 2.22E+01 0 -1.33E+01 0 0 0 -8.88E+00 0 0
PERT MJ 2.14E+02 5E-03 9E-02 2.21E+03 0 3E-03 6.41E-01 7.2E-02 -4.87E+01
PENRE MJ 7.36E+02 1.61E+00 4.95E-01 4.98E+03 0 8.36E-01 8.33E+01 5.5E-01 -1.9E+02
PENRM MJ 8.08E+01 0 0 0 0 0 -8.08E+01 0 0
PENRT MJ 8.17E+02 1.61E+00 4.95E-01 4.98E+03 0 8.36E-01 2.55E+00 5.5E-01 -1.9E+02
SM kg 5.66E+00 0 0 0 0 0 0 0 0
RSF MJ 0 0 0 0 0 0 0 0 0
NRSF MJ 0 0 0 0 0 0 0 0 0
FW m3 3.25E-01 9.08E-06 5E-03 2.55E+00 0 4.72E-06 1.5E-02 1.39E-04 -9.5E-02
PERE = Use of renewable primary energy excluding renewable primary energy resources used as raw materials; PERM = Use of renewable primary
energy resources used as raw materials; PERT = Total use of renewable primary energy resources; PENRE = Use of non-renewable primary energy
excluding non-renewable primary energy resources used as raw materials; PENRM = Use of non-renewable primary energy resources used as raw
materials; PENRT = Total use of non-renewable primary energy resources; SM = Use of secondary material; RSF = Use of renewable secondary fuels;
NRSF = Use of non-renewable secondary fuels; FW = Use of net fresh water
RESULTS OF THE LCA – WASTE CATEGORIES AND OUTPUT FLOWS according to EN 15804+A2:
1 piece UniSwing Compact / Robust / Fire
Parameter Unit A1-A3 A4 A5 B6 C1 C2 C3 C4 D
HWD kg 3.63E-05 1.56E-10 7.3E-10 2.06E-06 0 8.11E-11 8.81E-09 8.39E-09 -3.9E-06
NHWD kg 3.33E+00 1.64E-04 4.9E-02 3.54E+00 0 8.55E-05 5.16E-01 2.77E+00 -6.13E-01
RWD kg 2.8E-02 1.73E-06 2.6E-05 7.56E-01 0 8.97E-07 1E-04 6.26E-06 -1.3E-02
CRU kg 0 0 0 0 0 0 0 0 0
MFR kg 0 0 0 0 0 0 6.55E+00 0 0
MER kg 0 0 0 0 0 0 0 0 0
EEE MJ 0 0 2.37E+00 0 0 0 1.11E+01 0 0
EET MJ 0 0 4.3E+00 0 0 0 2.45E+01 0 0
4 Environmental Product Declaration - KONE - UniSwing Compact / Robust / Fire
HWD = Hazardous waste disposed; NHWD = Non-hazardous waste disposed; RWD = Radioactive waste disposed; CRU = Components for re-use;
MFR = Materials for recycling; MER = Materials for energy recovery; EEE = Exported electrical energy; EET = Exported thermal energy
RESULTS OF THE LCA – additional impact categories according to EN 15804+A2-optional:
1 piece UniSwing Compact / Robust / Fire
Parameter Unit A1-A3 A4 A5 B6 C1 C2 C3 C4 D
Disease
PM 2.07E-06 5.96E-10 2.43E-09 5.25E-06 0 3.1E-10 1.2E-08 3.72E-09 -6.78E-07
incidence
IR kBq U235 eq 3.34E+00 2.46E-04 4E-03 1.24E+02 0 1.28E-04 1E-02 6.44E-04 -2.1E+00
ETP-fw CTUe 3.71E+02 1.14E+00 2.35E-01 2.13E+03 0 5.92E-01 9.74E-01 3.14E-01 -6.43E+01
HTP-c CTUh 2.96E-08 2.14E-11 1.24E-11 5.89E-08 0 1.11E-11 8.17E-11 4.66E-11 2.28E-08
HTP-nc CTUh 1.55E-06 9.15E-10 5.38E-10 2.17E-06 0 4.76E-10 7.72E-09 5.13E-09 2.7E-06
SQP SQP 4.67E+02 4E-03 1.31E-01 1.59E+03 0 2E-03 7.57E-01 1.15E-01 -1.51E+01
PM = Potential incidence of disease due to PM emissions; IR = Potential Human exposure efficiency relative to U235; ETP-fw = Potential comparative
Toxic Unit for ecosystems; HTP-c = Potential comparative Toxic Unit for humans (cancerogenic); HTP-nc = Potential comparative Toxic Unit for humans
(not cancerogenic); SQP = Potential soil quality index
Disclaimer 1 – for the indicator “Potential Human exposure efficiency relative to U235”. This impact category deals mainly with the
eventual impact of low-dose ionizing radiation on human health of the nuclear fuel cycle. It does not consider effects due to possible
nuclear accidents, occupational exposure or radioactive waste disposal in underground facilities. Potential ionizing radiation from the
soil, radon and from some construction materials is also not measured by this indicator.
Disclaimer 2 – for the indicators “abiotic depletion potential for non-fossil resources”, “abiotic depletion potential for fossil resources”,
“water (user) deprivation potential, deprivation-weighted water consumption”, “potential comparative toxic unit for ecosystems”,
“potential comparative toxic unit for humans – cancerogenic”, “Potential comparative toxic unit for humans - not cancerogenic”,
“potential soil quality index”. The results of this environmental impact indicator shall be used with care as the uncertainties on these
results are high as there is limited experience with the indicator.
This EPD was created using a software tool.
References
ISO 14025
DIN EN ISO 14025:2011-10, Environmental labels and IBU 2021
declarations — Type III environmental declarations — General Instructions for the EPD programme of Institut Bauen
Principles and procedures. und Umwelt e.V. Version 2.0, Berlin: Institut Bauen und Umwelt
e.V., 2021. www.ibu-epd.com.
EN 15804
EN 15804+A2:2019+AC:2021, Sustainability of construction GaBi
works — Environmental Product Declarations — Core rules for Sphera Solutions GmbH Gabi Software System and Database
the product category ofconstruction products. for Life Cycle Engineering 1992-2020 Version 10.0.0.71
University of Stuttgart Leinfelden-Echterdingen.
EN 18650
EN 18650-1:2010, Powered pedestrian doors - Part 1: Product GaBi ts documentation
requirements and test methods. GaBi life cycle inventory data documentation
(https://www.gabisoftware.com/support/gabi/gabidatabase-
EN 18650 2020-lci-documentation/).
EN 18650-2:2010, Powered pedestrian doors - Part 2: Safety at
powered pedestrian doors. LCA-tool dormakaba
LCA tool, version ENS (drive system) Tool No.: IBU-DOR-
EN 16005 202108-LT1-EN Developed by Sphera Solutions GmbH.
EN 16005: 2013-01, Power operated pedestrian doorsets -
Safety in use - Requirements and test methods. PCR Part A
PCR – Part A: Calculation Rules for the Life Cycle Assessment
EN 60335 and Requirements on the Project Re-port according to EN
EN 60335-1, -2-103:2020-08, Household and similar electrical 15804+A2:2019, Version 1.0, Institut Bauen und Umwelt e.V.,
appliances - Safety - Part 1: General requirements. www.ibu-epd.com.
EN 61000 PCR Part B
EN 61000-1-2:2017-07, Electromagnetic compatibility (EMC) - PCR – Part B: Requirements on the EPD for Drive systems for
Part 1-2: General - Methodology for the achievement of automatic doors and gates, 08.2021, Institut Bauen und Umwelt
functional safety of electrical and electronic systems including e.V., www.ibu-epd.com.
equipment with regard to electromagnetic phenomena.
REACH
EN ISO 13849 Registration, Evaluation, Authorisation and Restriction of
EN ISO 13849-1:2021-08, Safety of machinery - Safety-related Chemicals (REACH), Regulation (EC) No 1907/2006.
parts of control systems - Part 1: General principles for design.
2011/65/EU ROHS3 Directive
Machinery Directive Directive 2011/65/EU of the European Parliament and of the
Directive 2006/42/EC of the European Parliament and of the Council of 8 June 2011 on the restriction of the use of certain
Council on machinery, and amending Directive 95/16/EC. hazardous substances in electrical and electronic equipment.
5 Environmental Product Declaration - KONE - UniSwing Compact / Robust / Fire
European Chemicals Agency (ECHA)
https:echa.europa.eu/de/home.
6 Environmental Product Declaration - KONE - UniSwing Compact / Robust / Fire
Publisher
Institut Bauen und Umwelt e.V. +49 (0)30 3087748- 0
Hegelplatz 1 info@ibu-epd.com
10117 Berlin www.ibu-epd.com
Germany
Programme holder
Institut Bauen und Umwelt e.V. +49 (0)30 3087748- 0
Hegelplatz 1 info@ibu-epd.com
10117 Berlin www.ibu-epd.com
Germany
Author of the Life Cycle Assessment
dormakaba International Holding GmbH +49 2333 793-0
DORMA Platz 1 info.de@dormakaba.com
58256 Ennepetal www.dormakaba.com
Germany
Owner of the Declaration
KONE Corporation +358(0)204 75 1
Keilasatama 3 contact@kone.com
02150 ESPOO www.kone.com
Finland
7 Environmental Product Declaration - KONE - UniSwing Compact / Robust / Fire
