ENVIRONMENTAL PRODUCT DECLARATION
as per ISO 14025 and EN 15804+A1
Owner of the Declaration Wallmann A/S
Publisher Institut Bauen und Umwelt e.V. (IBU)
Programme holder Institut Bauen und Umwelt e.V. (IBU)
Declaration number EPD-WAL-20220119-CBC2-EN
Issue date 06.05.2022
Valid to 05.05.2027
Wallmann "No Noise" underlag
Wallmann A/S
www.ibu-epd.com | https://epd-online.com
General Information
Wallmann A/S Wallmann "No Noise" underlag
Programme holder Owner of the declaration
IBU – Institut Bauen und Umwelt e.V. Wallmann A/S
Hegelplatz 1 Sabroesvej 20B
10117 Berlin 8600 Silkeborg
Germany Denmark
Declaration number Declared product / declared unit
EPD-WAL-20220119-CBC2-EN Polyurethane underlayment mats - 1 m2 polyurethane underlayment mats
with renewable plant oil
This declaration is based on the product category rules: Scope:
Floor coverings, 06.04.2023 The manufacturer declaration applies to a group of similar products with a
(PCR checked and approved by the SVR) minimum weight of 1 kg/m2 and a maximum total weight of 4 kg/m2.
The product is available as rolls and tiles. It is manufactured at the
Windmoller GmbH site in Detmold, Germany. LCA results for product
Issue date groups having a lower total weight than 4 kg/m2 can be taken from the
06.05.2022 corresponding tables of the annexe. Specific data can be calculated by
using equation 1 given in the annexe (see annexe chapter: 'General
Information on the annexe').
Valid to The owner of the declaration shall be liable for the underlying information
and evidence; the IBU shall not be liable with respect to manufacturer
05.05.2027 information, life cycle assessment data and evidences.
The EPD was created according to the specifications of EN 15804+A1. In
the following, the standard will be simplified as EN 15804.
Verification
The standard EN 15804 serves as the core PCR
Independent verification of the declaration and data according to ISO
14025:2011
internally X externally
Dipl.-Ing. Hans Peters
(Chairman of Institut Bauen und Umwelt e.V.)
Dipl.-Ing. Hans Peters Angela Schindler,
(Managing Director Institut Bauen und Umwelt e.V.) (Independent verifier)
1 Environmental-Product Declaration - Wallmann A/S - Wallmann "No Noise" underlag
Product
Performance data of the product can be found on the
Product description/Product definition manufacturer's technical information section
Underlayment mats based on polyurethane are produced with (www.wallmann.dk).
renewable plant oil and with natural inorganic filler. The mats
are available in different weights and thicknesses and are Base materials/Ancillary materials
offered as rolls or tiles. The declaration applies to a group of Name Value Unit
products with a minimum total weight of 1 kg/m2 and a Polyurethane including 73 % renewable material 18,4 %
maximum total weight of 4 kg/m². The mats consist of a
Inorganic Fillers 76,2 %
laminated polyurethane core.
Organic layers 4,6 %
LCA results for products with lower weights can be taken from Additives 0,8 %
the corresponding tables of the annexe. Results for specific This product contains substances listed in the ECHA candidate
products with total weights between 1 kg/m2 and 4 kg/m2 can list (19.01.2021) or other carcinogenic, mutagenic or reprotoxic
be calculated by using equation 1 given in the annexe (see (CMR) substances in categories 1A or 1B which are not on the
annexe chapter: 'General Information on the annexe'). For the candidate list exceeding 0.1 percentage by mass: no
placing on the market of the product in the European
Union/European Free Trade Association (EU/EFTA) (with the
exception of Switzerland) the technical requirements of the
underlayment mats are covered by EN 16354:2019-01. Reference service life
A calculation of the reference service life according to ISO
Application 15686 is not possible.
The products are applied below floor coverings. They can be The service life of the underlay mats strongly depends on the
used in domestic, commercial and industrial areas. correct installation. The service life of the declared underlay
mats is mainly dependent on the service life of the covering
Technical Data
layer.
A minimum service life of 10 years can be assumed, technical
Name Value Unit service life can be considerably longer.
Product Form mats -
Grammage 4000 kg/m2
Polyurethane layer 3833 g/m²
Lamination 167 g/m²
LCA: Calculation rules
and waste processing up to the landfill disposal of residual
Declared Unit waste
(except radioactive waste). Benefits for generated electricity
Name Value Unit and steam
Declared unit 1 m2 due to the incineration of production waste are aggregated.
Biogenic carbon that is stored in renewable material (plant oil,
Grammage 4 kg/m2
packaging paper) is taken into account as well as the
Layer thickness 0.002 m associated carbon dioxide uptake from the air during the growth
Gross density 2000 kg/m3 of the plants
The declared unit refers to 1 m2 produced underlay mat. The
A4 Transport:
output of module A5 'Assembly' is 1 m2 installed underlay mat.
Transport of the packed product from factory gate to the place
of installation.
A5 Installation:
System boundary
Installation
Type of EPD: Cradle-to-gate with options
of the floor covering, processing of installation waste and
packaging waste up to the landfill disposal of residual waste
System boundaries of modules A, B, C, D:
(except
Modules C3, C4 and D are indicated separately for three end-
radioactive waste), the production of the amount of underlay
of-life scenarios:
mat that occurs
1 - landfill disposal
as installation waste including its transport to the place of
2 - municipal waste incineration
installation.
3 - recovery in a cement plant
Generated electricity and steam due to the incineration of
waste are listed in the result table as exported energy.
A1-A3 Production:
Biogenic carbon that is stored in renewable materials the
Energy
polyurethane layer and in packaging paper is released as
supply and production of the basic material, processing of
carbon dioxide emissions into the air at the end of life in module
secondary
A5.
material, auxiliary material, transport of the material to the
manufacturing site, emissions, waste water treatment,
B1 - B7:
packaging material
The modules are not relevant and therefore not declared.
2 Environmental-Product Declaration - Wallmann A/S - Wallmann "No Noise" underlag
C1 De-construction: D Recycling potential:
The floor covering is de-constructed manually and no additional Calculated benefits result from materials exclusive secondary
environmental impact is caused. materials (net materials).
D-A5: Benefits for generated energy due to incineration of
C2 Transport: packaging and installation waste (incineration plant with R1 >
Transport 0.6),
of the underlay mat waste to a landfill, to the municipal waste D-1: Benefits for generated energy due to landfill disposal of
incineration underlay mat waste at the end-of-life,
plant (MWI) or to the waste collection facility for recycling. D-2: Benefits for generated energy due to incineration of
underlay mat waste at the end-of-life (incineration plant with
C3 Waste processing: R1 > 0.6),
C3-1: Landfill disposal needs no waste processing. D-3: Benefits for saved fossil energy and saved inorganic
C3-2: Impact from waste incineration (plant with material due to recovery of the underlay mat in a cement plant.
R1>0.6), generated electricity and steam are listed in the result
table as exported energy. Geographic Representativeness
C3-3: Collection of the underlay mat waste for recovery in the Land or region, in which the declared product system is
cement industry, waste processing (granulating), transport to manufactured, used or handled at the end of the product´s
the cement plant, emissions from the incineration. The biogenic lifespan: Europe
carbon that is stored in the renewable materials of the floor
covering is released into the air as carbon dioxide emissions.
Comparability
Basically, a comparison or an evaluation of EPD data is only
C4 Disposal
possible if all the data sets to be compared were created
C4-1: Impact from landfill disposal,
according to EN 15804 and the building context, respectively
C4-2: The underlay mat waste leaves the system in
the product-specific characteristics of performance, are taken
module C3-2,
into account. Background data are taken from GaBi database
C4-3: The pre-processed underlay mat waste leaves the
2021. Remaining data gaps are covered by the ecoinvent 3.7
system in module C3-3.
database.
LCA: Scenarios and additional technical information
should be done according to the following scheme:
The following information refer to the declared modules and are EOL-impact = x % impact (Scenario 1)
the basis for calculations or can be used for further calculations. + y % impact (Scenario 2)
+ z % impact (Scenario 3)
Transport to the construction site (A4)
with x % + y % + z % = 100 %
Name Value Unit
Litres of fuel (truck, EURO 0-6 mix) 0.0094 l/100km
Name ValueUnit
Transport distance 870 km
Collected as mixed construction waste (scenario 1
Capacity utilisation (including empty runs) 55 % and 2) 4 kg
Landfilling (scenario 1) 4 kg
Installation in the building (A5)
Energy recovery (scenario 2) 4 kg
Name Value Unit
Collected separately (scenario 3) 4 kg
Material loss 0.36 kg
Energy recovery (scenario 3) 0,941 kg
Polyethylene packaging waste and installation waste are
Recycling (scenario 3) 3.059 kg
considered to be incinerated in a municipal waste incineration
plant. Cardboard is going to be recycled.
Reuse, recovery and/or recycling potentials (D), relevant
scenario information
Recovery or recycling potentials due to the three end-of-life
End of Life (C1-C4)
scenarios (module C) are indicated separately.
Three different end-of-life scenarios are declared and the
results are indicated separately in module C.
Recycling in the cement industry (scenario 3)
Each scenario is calculated as a 100 % scenario.
VDZ e.V.
The organic material of the underlay mat is used as secondary
Scenario 1: 100 % landfill disposal
fuel in a cement kiln. It mainly substitutes for lignite (65.5 %),
Scenario 2: 100 % municipal waste incineration (MWI)
hard coal (26.2 %) and petrol coke (8.6 %).
with R1>0.6
The inorganic material is substantially integrated into the
Scenario 3: 100 % recycling in the cement industry
cement clinker and substitutes for original material input.
If combinations of these scenarios have to be calculated this
3 Environmental-Product Declaration - Wallmann A/S - Wallmann "No Noise" underlag
LCA: Results
The LCA results refer to all declared products with a maximum weight of 4000 g/m2. LCA results for products with lower weights can be
taken from the corresponding tables of the annexe. Results for specific products with weights between 1 kg/m2 and 4 kg/m2 can be
calculated by using equation 1 given in the annexe (see annexe chapter: 'General Information on the annexe'). Information on non-
relevant modules: Modules B1 - B7 are not relevant during the service life of the underlay mat. Modules C1, C3/1, C4/2 and C4/3
cause no additional impact (see chapter "LCA: Calculation rules" in this document). All these modules are declared and marked as
'modules not relevant/declared'. Module C2 represents the transport for scenarios 1, 2 and 3. Column D represents module D/A5. The
calculations are based on the CML characterization factors (version August 2016).
DESCRIPTION OF THE SYSTEM BOUNDARY (X = INCLUDED IN LCA; MND = MODULE NOT DECLARED; MNR = MODULE NOT
RELEVANT)
Benefits and
Construction loads beyond
Product stage Use stage End of life stage
process stage the system
boundaries
la ire ta m w a Ry lp p u s tro p s n a rT g n iru tc a fu n a M e h t m o rf tro p s n a rTe tis e h t o t e ta g y lb m e s s A e s U e c n a n e tn ia M ria p e R tn e m e c a lp e R tn e m h s ib ru fe R y g re n e la n o ita re p Oe s u re ta w la n o ita re p Oe s u n o itc u rts n o c -e Dn o itilo m e d tro p s n a rT g n is s e c o rp e ts a W la s o p s iD -e s u e R-y re v o c e R-g n ilc y c e Rla itn e to p
A1 A2 A3 A4 A5 B1 B2 B3 B4 B5 B6 B7 C1 C2 C3 C4 D
X X X X X MND MND MNR MNR MNR MND MND MND X X X X
RESULTS OF THE LCA - ENVIRONMENTAL IMPACT according to EN 15804+A1: 1 m² floorcovering
Parameter Unit A1-A3 A4 A5 C2 C3/2 C3/3 C4/1 D D/1 D/2 D/3
GWP kg CO 2 eq 8.42E-01 2.91E-01 4.96E-01 1.33E-02 4.1E+00 4.15E+00 1.79E+00 -6.52E-02 0 -6.23E-01 -2.41E-01
kg CFC11
ODP 1.59E-08 5.08E-17 1.43E-09 2.32E-18 1.83E-15 2.54E-15 9.22E-16 -9.56E-16 0 -9.05E-15 -1.12E-15
eq
AP kg SO 2 eq 1.86E-02 1.2E-03 1.9E-03 5.49E-05 1.17E-03 1.35E-03 7.05E-04 -7.36E-05 0 -6.99E-04 -5.29E-04
EP kg PO 43 eq 1.63E-02 3.06E-04 1.52E-03 1.4E-05 2.73E-04 3.13E-04 7.65E-04 -1.02E-05 0 -9.71E-05 -9.45E-05
POCP kg Ethen eq 2.89E-04 -5.15E-04 -1.5E-05 -2.35E-05 7.96E-05 2.39E-05 6.34E-05 -6.84E-06 0 -6.52E-05 -6.99E-05
ADPE kg Sb eq 4.12E-06 2.58E-08 3.89E-07 1.18E-09 1.85E-07 1.95E-07 5.21E-08 -1.19E-08 0 -1.13E-07 -2.85E-08
ADPF MJ 4.37E+01 3.96E+00 4.51E+00 1.81E-01 2.28E+00 2.97E+00 4.06E+00 -9.44E-01 0 -9.04E+00 -2.47E+01
GWP = Global warming potential; ODP = Depletion potential of the stratospheric ozone layer; AP = Acidification potential of land and water; EP =
Eutrophication potential; POCP = Formation potential of tropospheric ozone photochemical oxidants; ADPE = Abiotic depletion potential for non-fossil
resources; ADPF = Abiotic depletion potential for fossil resources
RESULTS OF THE LCA - INDICATORS TO DESCRIBE RESOURCE USE according to EN 15804+A1: 1 m² floorcovering
Parameter Unit A1-A3 A4 A5 C2 C3/2 C3/3 C4/1 D D/1 D/2 D/3
PERE MJ 2.69E+01 2.22E-01 2.56E+00 1.01E-02 4.43E-01 6.49E-01 3.03E-01 -2.47E-01 0 -2.33E+00 -2.57E-01
PERM MJ 7.4E-02 0 -7.4E-02 0 0 0 0 0 0 0 0
PERT MJ 2.7E+01 2.22E-01 2.49E+00 1.01E-02 4.43E-01 6.49E-01 3.03E-01 -2.47E-01 0 -2.33E+00 -2.57E-01
PENRE MJ 1.84E+01 3.97E+00 4.9E+00 1.81E-01 2.87E+01 2.96E+01 4.18E+00 -1.14E+00 0 -1.09E+01 -2.48E+01
PENRM MJ 2.64E+01 0 -2.58E-01 0 -2.62E+01 -2.62E+01 0 0 0 0 0
PENRT MJ 4.49E+01 3.97E+00 4.64E+00 1.81E-01 2.53E+00 3.38E+00 4.18E+00 -1.14E+00 0 -1.09E+01 -2.48E+01
SM kg 2.15E-02 0 1.94E-03 0 0 0 0 0 0 0 2.67E+00
RSF MJ 0 0 0 0 0 0 0 0 0 0 0
NRSF MJ 0 0 0 0 0 0 0 0 0 0 0
FW m3 2.19E+00 2.54E-04 1.98E-01 1.16E-05 1.33E-02 1.35E-02 3.85E-05 -2.41E-04 0 -2.28E-03 -1.95E-03
PERE = Use of renewable primary energy excluding renewable primary energy resources used as raw materials; PERM = Use of renewable primary
energy resources used as raw materials; PERT = Total use of renewable primary energy resources; PENRE = Use of non-renewable primary energy
excluding non-renewable primary energy resources used as raw materials; PENRM = Use of non-renewable primary energy resources used as raw
materials; PENRT = Total use of non-renewable primary energy resources; SM = Use of secondary material; RSF = Use of renewable secondary fuels;
NRSF = Use of non-renewable secondary fuels; FW = Use of net fresh water
RESULTS OF THE LCA – WASTE CATEGORIES AND OUTPUT FLOWS according to EN 15804+A1:
1 m² floorcovering
Parameter Unit A1-A3 A4 A5 C2 C3/2 C3/3 C4/1 D D/1 D/2 D/3
HWD kg 2.77E-05 2E-10 2.5E-06 9.14E-12 4.19E-10 5.46E-10 7.52E-10 -2.55E-10 0 -2.43E-09 -5.22E-10
NHWD kg 9.76E-02 5.9E-04 1.35E-01 2.69E-05 1.41E+00 1.41E+00 3.98E+00 -5.24E-04 0 -4.99E-03 -1.06E-03
RWD kg 4.26E-04 4.81E-06 4.8E-05 2.19E-07 1.01E-04 1.6E-04 4.85E-05 -7.93E-05 0 -7.5E-04 -4.8E-05
CRU kg 0 0 0 0 0 0 0 0 0 0 0
MFR kg 0 0 2.47E-02 0 0 2.67E+00 0 0 0 0 0
MER kg 0 0 0 0 0 0 0 0 0 0 0
EEE MJ 0 0 2.7E-01 0 2.56E+00 0 0 0 0 0 0
EET MJ 0 0 5.36E-01 0 5.17E+00 0 0 0 0 0 0
HWD = Hazardous waste disposed; NHWD = Non-hazardous waste disposed; RWD = Radioactive waste disposed; CRU = Components for re-use;
MFR = Materials for recycling; MER = Materials for energy recovery; EEE = Exported electrical energy; EET = Exported thermal energy
4 Environmental-Product Declaration - Wallmann A/S - Wallmann "No Noise" underlag
References
EN 13501-1 Regulation
DIN No. 305/2011 Construction Products Regulation (CPR) of the
EN 13501-1:2019-05: Fire classification of construction European
products and Council and of the European Parliament, April 2011
building elements - Part 1: Classification using data from
reaction to CML characterization factors
fire tests Impact assessment characterization factors, version 4.7,
August 2016, Institute of Environmental Sciences - 'Centrum
EN 14041 voor Milieuwetenschappen in Leiden' (CML), Leiden, The
DIN EN 14041: 2018-05: Resilient, textile and laminate floor Netherlands
coverings - Essential characteristics
ECHA candidate list
EN 15804 Candidate List of substances of very high concern (SVHCs) for
EN authorisation, 19.01.2021, European Chemicals Agency
15804:2012-04+A1 2013/, Sustainability of construction works (ECHA), Helsinki, Finland
—
Environmental Product Declarations — Core rules for the ecoinvent 3.7
product category ecoinvent, Zurich, Switzerland, database version 3.7, published
of construction products September 2020
EN 16354 GaBi database 2021
Laminate floor coverings - Underlays - Specification, GaBi Software-System and Database for Life Cycle
requirements and test methods Engineering, thinkstep AG, Leinfelden-Echterdingen, 2021-2
EN 16810 IBU 2021
DIN IBU
EN 16810: 2017-08: Resilient, textile and laminate floor (2021): General Programme Instructions for the Preparation of
coverings – EPDs at
Environmental product declarations – Product category rules the Institut Bauen und Umwelt e.V., Version 2.0 Institut Bauen
und
ISO 10874 Umwelt e.V., Berlin. www.ibu-epd.de
DIN EN ISO 10874: 2012+A1:2021-04: Resilient, textile and
laminate floor coverings - Classification PCR Part A
Product
ISO 14025 Category Rules for Construction Products from the range of
DIN Environmental Product Declarations. Part A: Calculation Rules
EN /ISO 14025:2011-10/, Environmental labels and for the
declarations — Type Life Cycle Assessment and Requirements on the Background
III environmental declarations — Principles and procedures Report, V1.9,
Berlin: Institut Bauen und Umwelt e.V. (IBU), Januar 2021
ISO 14040
DIN EN ISO 14040:2006+A1:2020 Environmental PCR Part B
management - Life cycle assessment - Principles and Product
framework Category Rules for Construction Products from the range of
Environmental Product Declarations of Institut Bauen und
ISO 14044 Umwelt (IBU),
DIN EN ISO 14044:2006+A1:2018+A2:2020 Environmental Part B: Requirements on the EPD for floor coverings, V1,
management - Life cycle assessment - Requirements and Berlin: Institut Bauen und Umwelt e.V. (IBU), April 2023
guidelines
REACH
ISO 15686 Regulation
ISO 15686: Buildings and constructed assets - (EC) No 1907/2006 of the European Parliament and of the
Service life planning Council of 18
ISO 15686-1: 2011-05: Part 1: General principles and December 2006 concerning the Registration, Evaluation,
framework Authorisation and
ISO 15686-2: 2012-05: Part 2: Service life prediction Restriction of Chemicals (REACH). Last update: 27.02.2020
procedures (Status:
ISO 15686-7: 2017-04: Part 7: Performance 27.06.2018)
evaluation for feedback of service life data
from practice VDZ e.V.
ISO 15686-8: 2008-06: Part 8: Reference service life Association of German Cement Works, Ed. Environmental Data
and service-life estimation of the German Cement Industry 2019
Regulation (EU) No. 305/2011
5 Environmental-Product Declaration - Wallmann A/S - Wallmann "No Noise" underlag
Publisher
Institut Bauen und Umwelt e.V. +49 (0)30 3087748- 0
Hegelplatz 1 info@ibu-epd.com
10117 Berlin www.ibu-epd.com
Germany
Programme holder
Institut Bauen und Umwelt e.V. +49 (0)30 3087748- 0
Hegelplatz 1 info@ibu-epd.com
10117 Berlin www.ibu-epd.com
Germany
Author of the Life Cycle Assessment
Gemeinschaft umweltfreundlicher Teppichboden +49 (0)241 96843 410
(GUT) e.V. mail@gut-ev.de
Schönebergstraße 2 www.gut-ev.org
52068 Aachen
Germany
Owner of the Declaration
Wallmann A/S +4587700900
Sabroesvej 20B info@wallmann.dk
8600 Silkeborg www.wallmann.dk
Denmark
6 Environmental-Product Declaration - Wallmann A/S - Wallmann "No Noise" underlag
