ENVIRONMENTAL PRODUCT DECLARATION
as per ISO 14025 and EN 15804+A1
Owner of the Declaration Interface Europe Manufacturing BV
Programme holder Institut Bauen und Umwelt e.V. (IBU)
Publisher Institut Bauen und Umwelt e.V. (IBU)
Declaration number EPD-INT-20210152-CBB2-EN
Issue date 19.10.2021
Valid to 13.09.2026
Modular carpet tiles with CQuest Bio backing
pile material: continues-dyed polyamide 6 with 100%
recycled content and a maximum total pile weight of 1500
g/m2
Interface®
www.ibu-epd.com | https://epd-online.com
Umwelt Produktdeklaration Name des Herstellers – Name des Produkts
General Information
Interface® Modular carpet tiles with CQuest
Bio backing
max. total pile material 1500 g/m2 with
100% recycled PA 6 and continues
dyed surface
Programme holder Owner of the declaration
IBU – Institut Bauen und Umwelt e.V. Interface Europe Manufacturing BV
Panoramastr. 1 Industrielaan 15
10178 Berlin 3925 ZG Scherpenzeel
Germany The Netherlands
Declaration number Declared product / declared unit
EPD-INT-20210152-CBB2-EN 1 m² tufted modular carpet tiles with CQuest Bio
backing (CQB) and a pile material of PA 6 with 100%
recycled content
This declaration is based on the product Scope:
category rules: The manufacturer declaration applies to modular
Floor coverings, 02/2018 carpet tiles with CQuest Bio backing and a total pile
(PCR checked and approved by the SVR) material of max. 1500 g/m2 PA 6 with 100% recycled
content. The products are tufted in Scherpenzeel, The
Netherlands, or in Craigavon, Ireland. Dyeing of the
Issue date
surface is performed externally. The dyed carpets are
19.10.2021
back coated in Scherpenzeel.
The declaration is only valid in conjunction with a valid
Valid to
GUT-PRODIS license of the product.
13.09.2026
LCA results for products with a maximum total pile
weight of 600 g/m2 can be taken from the
corresponding tables of the annexe. Specific data for
every product within the declared group of products in
relation to its total pile weight can be calculated by
using equation 1 given in the annexe (see annexe
chapter: 'General information on the annexe')
The owner of the declaration shall be liable for the
underlying information and evidence; the IBU shall not
be liable with respect to manufacturer information, life
cycle assessment data and evidences.
The EPD was created according to the specifications
of EN 15804+A1. In the following, the standard will be
simplified as EN 15804.
Verification
The standard EN 15804 serves as the core PCR
Independent verification of the declaration and data
according to ISO 14025:2010
Dipl. Ing. Hans Peters internally x externally
(chairman of Institut Bauen und Umwelt e.V.)
Dr. Alexander Röder Dr. Eva Schmincke
(Managing Director Institut Bauen und Umwelt e.V.)) (Independent verifier)
Product
Product description/Product definition CQuest Bio backing system: Backing compound based
Tufted modular carpet tiles having a surface pile of on wood resin, containing a recycled filler, glass-fleece
continues-dyed polyamide 6 with 100% recycled reinforcement and polypropylene covering fleece.
content and a CQuest Bio backing system. The minimum recycled content with a total pile weight
of 1500 g/m2 is 71%. The declaration applies to a
group if products with a maximum total pile weight of
1500 g/m2. LCA results for poducts with a maximum
2 Environmental Product Declaration Interface – Tufted modular carpet tiles with CQuest Bio backing, aqueous dyed
surface and a max. total pile material of 1500 g/m² PA 6 with 100% recycled content
total pile weight of 600 g/m2 can be taken from the essential characteristics according to EN 14041: 2018-
corresponding tables of the annexe. Results for 05, Resilient, textile and laminate floor coverings -
specific products with other total pile weights can be Essential characteristics.
calculated by using equation 1 given in the annexe Additional product properties in accordance with EN
(see annexe chapter: 'General information on the 1307 can be found on the Product Information System
annexe') PRODIS using the PRODIS registration number of the
For the placing on the market of the product in the product (www.pro-dis.info) or on the manufacturer's
European Union/European Free Trade Association technical information section (www.interface.com).
(EU/EFTA) (with the exception of Switzerland)
Regulation (EU) No. 305/2011 Construction Product Base materials/Ancillary materials
Regulation (CPR) applies. The product needs a
Declaration of Performance (DoP) taking into Name Value Unit
consideration EN 14041, Resilient, textile and laminate Polyamide 6 28,4 %
floor coverings - Essential characteristics, May 2018, Polyester 1,4 %
and the CE-marking. The DoP of the product can be Polypropylene 0,9 %
found on the manufacturer's technical information Limestone 48.0 %
section. For the application and use of the product the Aluminum hydroxide 6.4 %
respective national provisions apply. Ethylene vinyl acetate (EVA) 7.0 %
Wood resin 5.4 %
Application
Glass fibre 0.6 %
According to the use class as defined in EN 1307 the
Additives 1.9 %
products can be used in all professional areas which
require class 33 or less.
This product contains substances listed in the ECHA
candidate list (16.01.2020) or other carcinogenic,
mutagenic, reprotoxic (CMR) substances in categories
1A or 1B which are not on the candidate list exceeding
0.1 percentage by mass: no
Technical Data The products are registered in the GUT-PRODIS
The performance data listed in the DoP apply. Information System. The PRODIS system ensures the
compliance with limitations of various chemicals and
Constructional data Volatile Organic Compound (VOC)-emissions and a
Name Value Unit ban on the use of all substances that are listed as
Modular carpet tiles, 50 'Substances of Very High Concern' (SVHC) under
Product Form -
cm x 50 cm REACH.
Type of manufacture tufted carpet -
PA6 with 100% recycled Reference service life
Yarn type -
content A calculation of the reference service life according to
Colouration continuous dyed surface ISO 15686 is not possible.
Primary 76% PET & 24% PA6 The service life of textile floor coverings strongly
CQuest Bio backing, depends on the correct installation taking into account
Secondary backing heavy backing with textile - the declared use classification and the adherence to
bottom cleaning and maintenance instructions.
Total pile weight max. 1500 g/m² A minimum service life of 10 years can be assumed,
Total carpet weight max. 5360 g/m2 technical service life can be considerably longer.
Performance data of the product in accordance with
the declaration of performance with respect to its
LCA: Calculation rules
Declared Unit - 1 landfill disposal
- 2 municipal waste incineration
- 3 recovery in a cement plant
Name Value Unit
Declared unit 1 m2 A1-A3 Production:
Conversion factor to 1 kg 5.36 kg/m2 Energy supply and production of the basic material,
The declared unit refers to 1 m2 produced textile floor processing of secondary material, auxiliary material,
covering. The output of module A5 'Assembly' is 1 m2 transport of the material to the manufacturing site,
installed textile floor covering. emissions, waste water treatment, packaging material
and waste processing up to the landfill disposal of
residual waste (except radioactive waste). Benefits for
System boundary generated electricity and steam due to the incineration
of production waste are aggregated.
Type of EPD: Cradle-to-grave Biogenic carbon that is stored in renewable material
(wood resin, renewable additives, packaging paper) is
System boundaries of modules A, B, C, D: taken into account as well as the associated carbon
Modules C3, C4 and D are indicated separately for dioxide uptake from the air from which this biogenic
three end-of-life scenarios: carbon comes.
3 Environmental Product Declaration Interface – Tufted modular carpet tiles with CQuest Bio backing, aqueous dyed
surface and a max. total pile material of 1500 g/m² PA 6 with 100% recycled content
C3 Waste processing:
A4 Transport: C3-1: Landfill disposal needs no waste processing.
Transport of the packed textile floor covering C3-2: The impact from waste incineration (plant with
from factory gate to the place of installation. R1>0.6), generated electricity and steam are listed in
the result table as exported energy. The biogenic
A5 Installation: carbon that is stored in the renewable materials of the
Installation of the textile floor covering, processing of floor covering is released into the air as carbon dioxide
installation waste and packaging waste up to the emissions.
landfill disposal of residual waste (except radioactive C3-3: Collection of the carpet waste for recovery in the
waste), the production of the amount of carpet that cement industry, waste processing (granulating),
occurs as installation waste including its transport to transport to the cement plant, emissions from the
the place of installation. Generated electricity and incineration. The biogenic carbon that is stored in the
steam due to the incineration of waste are listed in the renewable materials of the floor covering is released
result table as exported energy. into the air as carbon dioxide emissions.
Biogenic carbon that is stored in renewable materials
in installation waste and packaging paper is released C4 Disposal
as carbon dioxide emissions into the air at the end of C4-1: Impact from landfill disposal. The biogenic
life in module A5. carbon that is stored in the renewable materials of the
Preparation of the floor and auxiliary materials floor covering is released into the air as carbon dioxide
(adhesives, fixing agents, PET connectors) are beyond emissions.
the system boundaries and not taken into account. C4-2: The carpet waste leaves the system in
module C3-2.
B1 Use: C4-3: The pre-processed carpet waste leaves the
Indoor emissions during the use stage. After the first system in module C3-3.
year, no product- related Volatile Organic Compound
(VOC) emissions are relevant due to known VOC D Recycling potential:
decay curves of the product. Calculated benefits result from materials exclusive
secondary materials (net materials).
B2 Maintenance:
Cleaning of the textile floor covering for a period of 1 D-A5: Benefits for generated energy due
year: to incineration of packaging and installation waste
Vacuum cleaning – electricity supply. (incineration plant with R1 > 0.6),
Wet cleaning – electricity, water consumption, D-1: Benefits for generated energy due to landfill
production of the cleaning agent, waste water disposal of carpet waste at the end-of-life,
treatment. D-2: Benefits for generated energy due to incineration
The declared values in this module have to be of carpet waste at the end-of-life (incineration plant
multiplied by the assumed service life of the floor with R1 > 0.6),
covering in the building in question. D-3: Benefits for saved fossil energy and saved
inorganic material due to recovery of the carpet in a
B3 - B7: cement plant.
The modules are not relevant and therefore not
declared. Comparability
Basically, a comparison or an evaluation of EPD data
C1 De-construction: is only possible if all the data sets to be compared
The floor covering is de-constructed manually and no were created according to EN 15804 and the building
additional environmental impact is caused. context, respectively the product-specific
characteristics of performance, are taken into account.
C2 Transport:
Transport of the carpet waste to a landfill, to the Background data are taken from the GaBi database
municipal waste incineration plant (MWI) or to the 2021-1 Remaining data gaps are covered by the
waste collection facility for recycling. ecoinvent 3.6 database 2019
LCA: Scenarios and additional technical information
The following information refer to the declared modules Polyethene packaging waste and installation waste are
and are the basis for calculations or can be used for considered to be incinerated in a municipal waste
further calculations. The indicated values refer to the incineration plant. Cardboard packaging waste is going
declared functional unit of all products with a total pile to be recycled.
weight up to 1300 g/m2. Preparation of the floor and auxiliaries (adhesives,
fixing agents, PET connectors, etc.) are not taken into
Transport to the construction site (A4) account.
Name Value Unit
Litres of fuel (truck, EURO 0-6 mix) 0.0126 l/100km
Transport distance 700 km
Capacity utilisation (incl. empty runs) 55 %
Maintenance (B2)
Installation in the building (A5)
The values for cleaning refer to 1 m2 floor covering
Name Value Unit
used in commercial areas per year. Depending on the
Material loss 0.16 kg
4 Environmental Product Declaration Interface – Tufted modular carpet tiles with CQuest Bio backing, aqueous dyed
surface and a max. total pile material of 1500 g/m² PA 6 with 100% recycled content
application based on ISO 10874, the technical service
life recommended by the manufacturer and the
anticipated strain on the floor by customers, the case-
specific useful life can be established. Based on this
useful life the effects of Module B2 need to be
calculated in order to obtain the overall environmental
impacts.
Name Value Unit
Maintenance cycle (wet cleaning) 1.5 1/year
Maintenance cycle (vacuum cleaning) 208 1/year
Water consumption (wet cleaning) 0.004 m3
Cleaning agent (wet cleaning) 0.09 kg
Electricity consumption 0.314 kWh
Further information on cleaning and maintenance see
www.interface.com
End of Life (C1-C4)
Three different end-of-life scenarios are declared and
the results are indicated separately in module C.
Each scenario is calculated as a 100% scenario.
Scenario 1: 100% landfill disposal
Scenario 2: 100% municipal waste incineration (MWI)
with R1>0.6
Scenario 3: 100% recycling in the cement industry
If combinations of these scenarios have to be
calculated this should be done according to the
following scheme:
EOL-impact = x% impact (Scenario 1)
+ y% impact (Scenario 2)
+ z% impact (Scenario 3)
with x% + y% + z% = 100%
Name Value Unit
Collected as mixed construction waste
5.36 kg
(scenario 1 and 2)
Collected separately (scenario 3) 5.36 kg
Landfilling (scenario 1) 5.36 kg
Energy recovery (scenario 2) 5.36 kg
Energy recovery (scenario 3) 2.414 kg
Recycling (scenario 3) 2.946 kg
Reuse, recovery and/or recycling potentials (D),
relevant scenario information
Recovery or recycling potentials due to the three end-
of-life scenarios (module C) are indicated separately.
Recycling in the cement industry (scenario 3)
VDZ e.V.
The organic material of the carpet is used as
alternative fuel in a cement kiln. It mainly substitutes
for lignite (64.5%), hard coal (26.5%) and petrol coke
(9.0%).
The inorganic material is substantially integrated into
the cement clinker and substitutes for original material
input.
5 Environmental Product Declaration Interface – Tufted modular carpet tiles with CQuest Bio backing, aqueous dyed
surface and a max. total pile material of 1500 g/m² PA 6 with 100% recycled content
LCA: Results
The LCA results refer to all declared products with a maximum total pile weight of 1500 g/m2. LCA results for
products with a maximum total pile weight of 600 g/m2 can be taken from the corresponding tables of the annexe.
Results for specific products with any other total pile weight can be calculated by using equation 1 given in the
annex (see annex chapter: 'General Information on the annex'). The declared result figures in module B2 have to
be multiplied by the assumed service life (in years) of the floor covering in the building under consideration.
Information on non-relevant modules: Modules B3 - B7 are not relevant during the service life of the carpet.
Modules C1, C3/1, C4/2 and C4/3 cause no additional impact (see chapter "LCA: Calculation rules" in this
document). All these modules are declared and marked as 'modules not relevant/declared'. Module C2 represents
the transport for scenarios 1, 2 and 3. Column D represents module D/A5. The calculations are based on the CML
characterization factors (version August 2016).
DESCRIPTION OF THE SYSTEM BOUNDARY (X = INCLUDED IN LCA; MND = MODULE NOT DECLARED;
MNR = MODULE NOT RELEVANT)
BENEFITS AND
CONSTRUCTI LOADS
PRODUCT STAGE ON PROCESS USE STAGE END OF LIFE STAGE BEYOND THE
STAGE SYSTEM
BOUNDARIES
6 Environmental Product Declaration Interface – Tufted modular carpet tiles with CQuest Bio backing, aqueous dyed
surface and a max. total pile material of 1500 g/m² PA 6 with 100% recycled content
lairetam
waR
ylppus tropsnarT
gnirutcafunaM
eht
morf
tropsnarT
etis
eht
ot
etag
ylbmessA esU
ecnanetniaM
riapeR
tnemecalpeR tnemhsibrufeR
ygrene
lanoitarepO esu
retaw
lanoitarepO esu
noitcurtsnoc-eD
noitilomed tropsnarT
gnissecorp
etsaW
lasopsiD -esueR -yrevoceR -gnilcyceR laitnetop
A1 A2 A3 A4 A5 B1 B2 B3 B4 B5 B6 B7 C1 C2 C3 C4 D
X X X X X X X MNR MNR MNR MND MND MND X X X X
RESULTS OF THE LCA - ENVIRONMENTAL IMPACT according to EN 15804+A1: 1 m² floorcovering
Parameter Unit A1-A3 A4 A5 B1 B2 C2 C3/2 C3/3 C4/1 D D/1 D/2 D/3
GWP [kg CO2-Eq.] 5.26E+0 3.19E-1 5.93E-1 0.00E+0 2.91E-1 4.45E-2 7.03E+0 7.11E+0 1.26E+0 -1.95E-2 0.00E+0 -3.27E-1 -2.42E-1
-2.99E- -4.93E- -1.46E-
ODP [kg CFC11-Eq.] 2.74E-8 5.56E-178.22E-100.00E+0 1.21E-8 7.76E-182.55E-153.50E-151.24E-15 0.00E+0
16 15 15
AP [kg SO2-Eq.] 2.33E-2 1.32E-3 8.93E-4 0.00E+0 1.14E-3 1.84E-4 4.99E-3 5.24E-3 9.44E-4 -2.27E-5 0.00E+0 -3.75E-4 -8.63E-4
EP [kg (PO4)3--Eq.] 5.95E-3 3.36E-4 2.27E-4 0.00E+0 3.17E-4 4.68E-5 1.26E-3 1.31E-3 1.03E-3 -3.11E-6 0.00E+0 -5.17E-5 -1.14E-4
POCP [kg ethene-Eq.] 1.42E-3 -5.64E-4 3.37E-5 6.29E-5 1.47E-4 -7.88E-5 3.03E-4 2.28E-4 8.50E-5 -2.08E-6 0.00E+0 -3.46E-5 -8.03E-5
ADPE [kg Sb-Eq.] 9.95E-6 2.83E-8 3.06E-7 0.00E+0 4.43E-6 3.94E-9 2.31E-7 2.45E-7 6.99E-8 -3.67E-9 0.00E+0 -6.07E-8 -1.90E-7
ADPF [MJ] 1.07E+2 4.34E+0 3.48E+0 0.00E+0 6.77E+0 6.06E-1 3.85E+0 4.79E+0 5.44E+0 -2.81E-1 0.00E+0-4.71E+0-2.16E+1
GWP = Global warming potential; ODP = Depletion potential of the stratospheric ozone layer; AP = Acidification potential of land and water; EP =
Caption Eutrophication potential; POCP = Formation potential of tropospheric ozone photochemical oxidants; ADPE = Abiotic depletion potential for non-
fossil resources; ADPF = Abiotic depletion potential for fossil resources
RESULTS OF THE LCA - INDICATORS TO DESCRIBE RESOURCE USE according to EN 15804+A1: 1 m²
floorcovering
Parameter Unit A1-A3 A4 A5 B1 B2 C2 C3/2 C3/3 C4/1 D D/1 D/2 D/3
PERE [MJ] 8.49E+1 2.43E-1 3.37E+0 0.00E+0 1.24E+0 3.39E-2 1.47E+1 1.49E+1 4.06E-1 -7.71E-2 0.00E+0 -1.27E+0 -3.42E-1
PERM [MJ] 1.44E+1 0.00E+0 -3.63E-1 0.00E+0 0.00E+0 0.00E+0 -1.41E+1 -1.41E+1 0.00E+0 0.00E+0 0.00E+0 0.00E+0 0.00E+0
PERT [MJ] 9.94E+1 2.43E-1 3.01E+0 0.00E+0 1.24E+0 3.39E-2 5.99E-1 8.75E-1 4.06E-1 -7.71E-2 0.00E+0 -1.27E+0 -3.42E-1
PENRE [MJ] 1.05E+2 4.35E+0 3.95E+0 0.00E+0 7.86E+0 6.07E-1 1.29E+1 1.40E+1 5.60E+0 -3.43E-1 0.00E+0 -5.74E+0 -2.18E+1
PENRM [MJ] 8.95E+0 0.00E+0 -2.75E-1 0.00E+0 0.00E+0 0.00E+0 -8.68E+0 -8.68E+0 0.00E+0 0.00E+0 0.00E+0 0.00E+0 0.00E+0
PENRT [MJ] 1.14E+2 4.35E+0 3.67E+0 0.00E+0 7.86E+0 6.07E-1 4.21E+0 5.34E+0 5.60E+0 -3.43E-1 0.00E+0 -5.74E+0 -2.18E+1
SM [kg] 4.28E+0 0.00E+0 1.28E-1 0.00E+0 0.00E+0 0.00E+0 0.00E+0 0.00E+0 0.00E+0 0.00E+0 0.00E+0 0.00E+0 2.60E-1
RSF [MJ] 0.00E+0 0.00E+0 0.00E+0 0.00E+0 0.00E+0 0.00E+0 0.00E+0 0.00E+0 0.00E+0 0.00E+0 0.00E+0 0.00E+0 0.00E+0
NRSF [MJ] 0.00E+0 0.00E+0 0.00E+0 0.00E+0 0.00E+0 0.00E+0 0.00E+0 0.00E+0 0.00E+0 0.00E+0 0.00E+0 0.00E+0 0.00E+0
FW [m³] 4.93E-1 2.78E-4 1.55E-2 0.00E+0 4.13E-3 3.88E-5 2.03E-2 2.06E-2 5.16E-5 -7.53E-5 0.00E+0 -1.24E-3 -2.06E-3
PERE = Use of renewable primary energy excluding renewable primary energy resources used as raw materials; PERM = Use of
renewable primary energy resources used as raw materials; PERT = Total use of renewable primary energy resources; PENRE = Use of
non-renewable primary energy excluding non-renewable primary energy resources used as raw materials; PENRM = Use of non-
Caption
renewable primary energy resources used as raw materials; PENRT = Total use of non-renewable primary energy resources; SM = Use
of secondary material; RSF = Use of renewable secondary fuels; NRSF = Use of non-renewable secondary fuels; FW = Use of net fresh
water
RESULTS OF THE LCA – WASTE CATEGORIES AND OUTPUT FLOWS according to EN 15804+A1:
1 m² floorcovering
Parameter Unit A1-A3 A4 A5 B1 B2 C2 C3/2 C3/3 C4/1 D D/1 D/2 D/3
HWD [kg] 4.23E-3 2.19E-10 1.27E-4 0.00E+0 5.90E-10 3.06E-11 1.69E-8 1.71E-8 1.01E-9 -7.70E-11 0.00E+0 -1.29E-9 -1.67E-9
NHWD [kg] 8.09E-1 6.47E-4 6.87E-2 0.00E+0 5.62E-3 9.02E-5 1.48E+0 1.48E+0 5.34E+0 -1.61E-4 0.00E+0 -2.67E-3 -1.62E-1
RWD [kg] 2.19E-3 5.27E-6 7.03E-5 0.00E+0 3.32E-4 7.35E-7 1.42E-4 2.21E-4 6.50E-5 -2.48E-5 0.00E+0 -4.09E-4 -8.83E-5
CRU [kg] 0.00E+0 0.00E+0 0.00E+0 0.00E+0 0.00E+0 0.00E+0 0.00E+0 0.00E+0 0.00E+0 0.00E+0 0.00E+0 0.00E+0 0.00E+0
MFR [kg] 0.00E+0 0.00E+0 1.21E-1 0.00E+0 0.00E+0 0.00E+0 0.00E+0 1.70E+0 0.00E+0 0.00E+0 0.00E+0 0.00E+0 0.00E+0
MER [kg] 0.00E+0 0.00E+0 0.00E+0 0.00E+0 0.00E+0 0.00E+0 0.00E+0 0.00E+0 0.00E+0 0.00E+0 0.00E+0 0.00E+0 0.00E+0
EEE [MJ] 0.00E+0 0.00E+0 2.78E-1 0.00E+0 0.00E+0 0.00E+0 7.85E+0 0.00E+0 0.00E+0 0.00E+0 0.00E+0 0.00E+0 0.00E+0
EET [MJ] 0.00E+0 0.00E+0 5.17E-1 0.00E+0 0.00E+0 0.00E+0 1.47E+1 7.45E+1 0.00E+0 0.00E+0 0.00E+0 0.00E+0 0.00E+0
HWD = Hazardous waste disposed; NHWD = Non-hazardous waste disposed; RWD = Radioactive waste disposed; CRU = Components
Caption for re-use; MFR = Materials for recycling; MER = Materials for energy recovery; EEE = Exported electrical energy; EET = Exported
thermal energy
The recycled content of the substance ethylene vinyl acetate (EVA) is calculated as virgin EVA because the
information on the specific recycling processes are not available.
Information on the biogenic carbon content: The textile floor covering contains renewable materials with stored
biogenic carbon. During the growth phase of plants carbon dioxide (CO ) is absorbed and transformed into stored
2
biogenic carbon. This amount of CO uptake is taken into account in module A1-A3 as a negative value that
2
reduces the total amount of the GWP. At the end of life the same amount of CO is released into the air as
2
emissions. These CO emissions increase the amount of the GWP in the three scenarios landfill disposal,
2
municipal incineration and recovery in the cement industry.
Biogenic carbon content per m2 textile floor covering: 0.27 kg C
Corresponding carbon dioxide uptake/emissions: 0.99 kg CO
2
Not all of the life cycle inventories applied in this study support the methodological approach for the waste and
water indicators. The data are based on publications of industry. The indicators for waste and water of the system
are evaluated but contain a higher degree of uncertainty.
References
EN 1307 ECHA candidate list
DIN EN 1307: 2014+A1:2016: Textile floor coverings - Candidate List of substances of very high concern
Classification (SVHCs) for authorisation, 16.01.2020, European
EN 13501-1 Chemicals Agency (ECHA), Helsinki, Finland
DIN EN 13501-1:2010-01: Fire classification of ecoinvent 3.6
construction products and building elements - Part 1: ecoinvent, Zurich, Switzerland, database version 3.6,
Classification using data from reaction to fire tests published September 2019
EN 14041 GaBi database 2021-1
DIN EN 14041: 2018-05: Resilient, textile and laminate GaBi Software-System and Database for Life Cycle
floor coverings - Essential characteristics Engineering, thinkstep AG, Leinfelden-Echterdingen,
EN 15804 2021-1
EN 15804:2012-04+A1 2013/, Sustainability of IBU 2021
construction works — Environmental Product IBU (2021): General Programme Instructions for the
Declarations — Core rules for the product category of Preparation of EPDs at the Institut Bauen und Umwelt
construction products e.V., Version 2.0 Institut Bauen und Umwelt e.V.,
EN 16810 Berlin, www.ibu-epd.de
DIN EN 16810: 2017-08: Resilient, textile and laminate PCR Part A
floor coverings – Environmental product declarations – Product Category Rules for Construction Products
Product category rules from the range of Environmental Product Declarations.
ISO 10874 Part A: Calculation Rules for the Life Cycle
DIN EN ISO 10874: 2012-04: Resilient, textile and Assessment and Requirements on the Background
laminate floor coverings - Classification Report, V1.9, Berlin: Institut Bauen und Umwelt e.V.
ISO 14025 (IBU), Januar 2021
DIN EN /ISO 14025:2011-10: Environmental labels PCR Part B
and declarations — Type III environmental Product Category Rules for Construction Products
declarations — Principles and procedures from the range of Environmental Product Declarations
ISO 15686 of Institut Bauen und Umwelt (IBU),
ISO 15686: Buildings and constructed assets - Part B: Requirements on the EPD for floor coverings,
Service life planning V1.2, Berlin: Institut Bauen und Umwelt e.V. (IBU),
ISO 15686-1: 2011-05: Part 1: General principles and February 2018
framework PRODIS
ISO 15686-2: 2012-05: Part 2: Service life prediction Product Information System (PRODIS) of the
procedures European Carpet Industry, Gemeinschaft
ISO 15686-7: 2006-03: Part 7: Performance umweltfreundlicher Teppichboden e.V (GUT) and
evaluation for feedback of service life data European Carpet and Rug Association
from practice (ECRA), http://www.pro-dis.info
ISO 15686-8: 2008-06: Part 8: Reference service life REACH
and service-life estimation Regulation (EC) No 1907/2006 of the European
Regulation (EU) No. 305/2011 Parliament and of the Council of 18 December 2006
Regulation No. 305/2011 Construction Products concerning the Registration, Evaluation, Authorisation
Regulation (CPR) of the European Council and of the and Restriction of Chemicals (REACH). Last update:
European Parliament, April 2011 27.02.2020
CML characterization factors VDZ e.V.
Impact assessment characterization factors, version Association of German Cement Works, Ed. Environ-
4.7, August 2016, Institute of Environmental Sciences - mental Data of the German Cement Industry 2018
'Centrum voor Milieuwetenschappen in Leiden' (CML),
Leiden, The Netherlands
7 Environmental Product Declaration Interface – Tufted modular carpet tiles with CQuest Bio backing, aqueous dyed
surface and a max. total pile material of 1500 g/m² PA 6 with 100% recycled content
Publisher
Institut Bauen und Umwelt e.V. Tel +49 (0)30 3087748- 0
Panoramastr. 1 Fax +49 (0)30 3087748- 29
10178 Berlin Mail info@ibu-epd.com
Germany Web www.ibu-epd.com
Programme holder
Institut Bauen und Umwelt e.V. Tel +49 (0)30 - 3087748- 0
Panoramastr 1 Fax +49 (0)30 – 3087748 - 29
10178 Berlin Mail info@ibu-epd.com
Germany Web www.ibu-epd.com
Author of the Life Cycle
Assessment Tel +49 (0)241 96843 410
Gemeinschaft umweltfreundlicher Fax +49 (0)241 96843 400
Teppichboden (GUT) e.V. Mail mail@gut-ev.de
Schönebergstraße 2 Web www.gut-ev.org
52068 Aachen
Germany
Owner of the Declaration
Interface Europe Manufacturing Tel +31 33 277 55 55
BV Fax +31 33 277 55 54
Industrielaan 15 Mail receptie@interface.com
3925ZG Scherpenzeel Web www.interface.com
Netherlands
