ENVIRONMENTAL PRODUCT DECLARATION
as per ISO 14025 and EN 15804+A2
Owner of the Declaration Sonae Arauco, S.A.
Publisher Institut Bauen und Umwelt e.V. (IBU)
Programme holder Institut Bauen und Umwelt e.V. (IBU)
Declaration number EPD-SON-20220210-ICC2-EN
Issue date 06.09.2022
Valid to 05.09.2027
AGEPAN® Wood Fibreboards
Sonae Arauco, S.A.
www.ibu-epd.com | https://epd-online.com
1. General Information
Sonae Arauco, S.A. AGEPAN® Wood Fibreboards
Programme holder Owner of the declaration
IBU – Institut Bauen und Umwelt e.V. Sonae Arauco, S.A.
Hegelplatz 1 Centro Empresarial Euronova, C/Ronda de Poniente, 6 ­ B
10117 Berlin 28760 Tres Cantos (Madrid)
Germany Spain
Declaration number Declared product / declared unit
EPD­SON­20220210­ICC2­EN AGEPAN® Wood Fibreboards, uncoated, per m3
This declaration is based on the product category rules: Scope:
Wood­based panels, 01.08.2021 This document refers to AGEPAN® Wood Fibreboards manufactured in the
(PCR checked and approved by the SVR) following plant of the Sonae Arauco group:
Sonae Arauco Deutschland GmbH
Issue date Meppen Plant
Grecostrasse 1
06.09.2022
49716 Meppen
Germany
Valid to
The production volume of this plant covers 100 % of the total production of
05.09.2027 AGEPAN® Wood Fibreboards by Sonae Arauco group.
The owner of the declaration shall be liable for the underlying information
and evidence; the IBU shall not be liable with respect to manufacturer
information, life cycle assessment data and evidences.
The EPD was created according to the specifications of EN 15804+A2. In
the following, the standard will be simplified as EN 15804.
Verification
The standard EN 15804 serves as the core PCR
Independent verification of the declaration and data according to ISO
Dipl.­Ing. Hans Peters 14025:2011
(Chairman of Institut Bauen und Umwelt e.V.)
internally X externally
Florian Pronold Dr. Stefan Diederichs,
(Managing Director Institut Bauen und Umwelt e.V.) (Independent verifier)
1 Environmental Product Declaration ­ Sonae Arauco, S.A. ­ AGEPAN® Wood Fibreboards
2. Product
2.1 Product description/Product definition
AGEPAN® System Wood Fiberboards are panel­shaped wood­
based materials in accordance with EN 316 that are
manufactured in a dry process by means of compression under
heat of wood fibres with adhesive. AGEPAN® System boards
can be blunt edged or profiled. Owing to their various densities
and adhesive systems, they can display a variety of material
properties:
• AGEPAN® THD is a wood fibre insulating panel with an
asymmetric density profile, manufactured in a dry
process.
• AGEPAN® THD Static is a wood fibre insulation board
with an asymmetrical bulk density profile and load­
bearing capacities.
• AGEPAN® DWD boards are permeable wall and roof Note:
boards manufactured in dry process with and without The legend for the acronyms used in the table above can be
tongue and groove profiles. found in the German standard DIN 4108-10:2008-06.
• AGEPAN® DWD 600 is a vapour­permeable wood fibre
board ideal for sheathing in rear­ventilated facades and
a second water­repellent layer in roof and wall.
• AGEPAN® UDP is another wood fibre insulation board
in our construction system for quick and easy working.
• AGEPAN® TEP is a wood fibre insulation board with an
asymmetric density profile and provides good technical
values and simple processing.
For the placing on the market of the product in the European
Union/European Free Trade Association (EU/EFTA) (with the
exception of Switzerland) Regulation (EU) No. 305/2011 (CPR)
applies. The product needs a declaration of performance taking
into consideration EN 13171:2008, Thermal insulation products
for buildings – Factory made wood fibre (WF) products –
Specification and the CE­marking.
For the application and use the respective national provisions
apply.
2.2 Application
AGEPAN® THD for windproof, heat­insulating, vapour
permeable and noise­insulating planking in roof and wall areas.
AGEPAN® THD Static for prefabricated elements for site
assembly and bare­bone houses with load­bearing capacities
(planking of in­plane loaded wall panels).
AGEPAN® DWD for reinforcement of timber frame
constructions as a stable panel and second water­bearing layer
in roof and wall.
AGEPAN® DWD 600 for sheathing in rear­ventilated facades,
second water­repellent layer in roof and wall and for approved
fire resistance construction in the Agepan System.
AGEPAN® UDP for exterior planking in roof and walls as a
second waterproof layer in various constructions.
AGEPAN® TEP for dry screed constructions as a direct
underlay for floating floorings.
Source:
DIN 4108-10:2008-06, Technische Baubestimmungen, DVD,
Stand 02/2015; Verlagsgesellschaft Rudolf Müller; Köln.
2.3 Technical Data
Values cover the range of uncoated AGEPAN® Wood
Fiberboards produced by Sonae Arauco Deutschland GmbH.
(see tables below).
Values cover the range of uncoated AGEPAN®
Wood Fiberboards produced by Sonae Indústria / Glunz AG
(see table above).
2 Environmental Product Declaration ­ Sonae Arauco, S.A. ­ AGEPAN® Wood Fibreboards
Name Value Unit
Gross density according to EN 323 210 ­ 650 kg/m3
Bending strength (longitudinal) according to
14 ­ 23 N/mm2
EN 310
1900 ­
E­module (longitudinal) according to EN 310 N/mm2
2700
Thermal conductivity according to EN 12524 0.14 W/(mK)
Water vapour diffusion resistance factor
3 ­ 12 ­
according to DIN 52615
Moisture content at delivery according to EN
4 ­ 9 %
322
Tensile strenght perpendicular to the plan 0.18 ­
N/mm2
according to EN 319 0.65
Performance data of the product in accordance with the 2.4 Delivery status
declaration of performance with respect to its essential AGEPAN® Wood Fibreboards ranging in thickness from 16 to
characteristics according to: 80 mm are procured as uncoated boards. The boards are
offered in standard formats.
• EN 13171:2008, Thermal insulation products for
Customized formats can also be available and selected formats
buildings – Factory made wood fibre (WF) products –
are offered with a tongue and groove profile.
Specification.
Information on dimensions can be seen in the table included in
• EN 13986:2004+A1:2015, Wood-based panels for
2.3 (above).
use in construction - Characteristics, evaluation of
For updated information on available dimensions, please refer
conformity and marking.
to www.sonaearauco.com
3 Environmental Product Declaration ­ Sonae Arauco, S.A. ­ AGEPAN® Wood Fibreboards
2.5 Base materials/Ancillary materials
AGEPAN® Wood Fibreboards consist of (dimensions as % by
mass):
• Wood chips, approx. 90 %
• Water, approx. 5­9 %
• PMDI glue (4.4' diphenylmethane diisocyanate), approx.
3.5 %
• Paraffin wax emulsion, 0.5­3 %
Wood from indigenous, largely regional forestry plantations is
used for manufacturing raw AGEPAN® Wood Fiberboards.
Wood certified in accordance with PEFC™ and FSC® schemes
is given preference in the range selection.
Furthermore, sawmill residues are also used in the production
of AGEPAN® Wood Fibreboards.
This product contains substances listed in the ECHA candidate
list (date: 08.06.2021) exceeding 0.1 percentage by mass:
• no 2.7 Environment and health during manufacturing
This product contains other carcinogenic, mutagenic or
Health protection: The manufacturing conditions do not
reprotoxic (CMR) substances in categories 1A or 1B which are
demand any special measures as regards health protection.
not on the ECHA candidate list, exceeding 0.1 percentage by
The reference occupational exposure limit values are complied
mass:
with.
• no
Biocide products were added to this construction product or it Emissions into air: Waste air generated during production is
has been treated with biocide products (this then concerns a cleaned in accordance with regulatory specifications. Emissions
treated product as defined by the (EU) Ordinance on Biocide are below the limit values specified by the operation license of
Products No. 528/2012: the site, specified according to German law.
• no
Emissions into water/soil: No contamination of water or soil.
2.6 Manufacture Waste water generated by production is treated and directed
The manufacturing of AGEPAN® Wood Fibreboards comprises into the municipal sewage system following pre­purification.
Sludge generated during water treatment is used in agriculture
the following steps:
as a fertilizer.
• Debarking the logs
• Chipping the wood to chips of approx. 3 x 3 cm in size
Noise: Sound protection analyses have established that all
• Boiling the chips
values communicated inside and outside the production
• Defibring in the refiner
facilities are below the standards applicable in Germany. Noise­
• Glueing the fibres with synthetic resin
intensive plant areas such as chipping are encapsulated
• Drying the fibres to an approx. moisture of 4% to 8%
appropriately by structural measures.
• Scattering the dried and glued fibre on a forming belt
The production site is ISO 14001 certified.
• Pressing the fibre mat in a continuous hot press under
high pressure 2.8 Product processing/Installation
• Cooling AGEPAN Wood Fibreboards can be sawn, milled, planed,
• Staking for stabilization sanded and drilled using standard machinery. Please refer to
• Cooling the respective data sheets for processing recommendations.
• Staking and Packing Correct structural installation must be ensured. When selecting
A process diagram is presented below. additional products, please ensure that they do not have a
negative influence on the designated environmental
Note: Sanding stage is represented in the diagram since it compatibility properties of the building products referred to.
exists in the plant, but is not used currently for AGEPAN
fibreboards production 2.9 Packaging
AGEPAN® Wood Fibreboards are supplied packed with
The production site is certified according to the following supporting timbers made of chipboard or medium­denistiy
standards: fibreboard (MDF), bundled with plastic made of recycled
polyethylene terephthalate (PET) (PET bottles) and covered
• ISO 9001
with cardboard.
• ISO 45001
• EN ISO 50001
The film for wrapping the T + G materials is made of recyclable
Additionally, all range includes CE marked products, and
low­density polyethylene.
PEFC™ and FSC® certified products can be made available on
request.
If re­use or recycling is impractical, the packaging should not be
landfilled, but rather directed towards energy recovery.
2.10 Condition of use
The components making up uncoated AGEPAN® Wood
Fibreboards correspond with the base material compositions as
outlined in Clause 2.5. During hot pressing, the binding agent
chemically reacts irreversibly by means of poly­condensation
4 Environmental Product Declaration ­ Sonae Arauco, S.A. ­ AGEPAN® Wood Fibreboards
and firmly bonded with the wood. The binding agents are For all other AGEPAN® Wood Fibreboards the classification is
chemically and stably bound to the wood. E.
VOC emissions: AGEPAN® Wood Fibreboards are labelled as
class A+ according to the French regulation on the labelling of
emissions of volatile compounds from construction and
decoration products (with reference to the wall scenario, as a Water
worst case). No ingredients are washed out which could be hazardous to
water. AGEPAN® Wood Fibreboards are not resistant to
Additionally, AGEPAN® Wood Fibreboards have been certified permanent exposure to water; damaged areas can however be
with the IBU environmental quality label. replaced locally.
Carbon storage: Mechanical destruction
AGEPAN® Wood Fibreboards at an average density of 464.2 AGEPAN® Wood Fibreboards breakage features display
kg/m3 stores 775 kg CO ­eq/m3 over their service life. relatively brittle performance, whereby sharp edges can arise
2
on the broken panel edges (risk of injury).
2.11 Environment and health during use
2.14 Re-use phase
Environmental protection: According to current information,
water, air and soil are not exposed to any dangers when the Recycling: AGEPAN® Wood Fibreboards from construction
respective products outlined above are used as designated. can be collected separately and utilized in the manufacture of
particleboard. This is based on the condition that the wooden
Health protection: According to current information, no boards are not fully glued.
damage to or impairment of health can be anticipated when
AGEPAN® Wood Fibreboards are used as designated. Energy recovery: due to the high heating value of approx. 16.6
MJ/kg at a 20 % moisture content assumed for post­consumer
VOC emissions at very low levels are basically composed of
natural wood ingredients. boards, AGEPAN® Wood Fibreboards can be used for energy
recovery and the generation of heat and electricity (e.g. in CHP
2.12 Reference service life plants), following the cascading principle for wood use.
Due to the wide range of applications of AGEPAN® Wood
2.15 Disposal
Fiberboards, no reference service life is declared.
AGEPAN® Wood Fibreboards leftovers and residual materials
2.13 Extraordinary effects incurred as a result of demolition measures on the building site
Fire should be primarily directed towards material recycling. If this is
Fire retardant classification of AGEPAN® Wood Fibreboards is not possible, they must be directed toward energy recovery
done according to EN 13171. Fire retardant classes are defined instead of landfilling.
in accordance with EN 13501-1.
Fire protection (for DWD (for DWD 600)): Waste code according to the European List of Waste: 17 02 01
Name Value 2.16 Further information
Building material class D Further information such as technical datasheets etc. can be
Smoke gas development s1 (s2) downloaded under:
Burning droplets d0
www.sonaearauco.com
3. LCA: Calculation rules
neglected.
3.1 Declared Unit The resource aspects of wood were inventoried via material
The declared unit for the LCA is 1 m3 of AGEPAN® Wood inherent properties such as resource extraction of CO from the
2
Fibreboard.The declared unit represents an average product, atmosphere and the lower heating value as the use of
calculated as the weighted average of the production volumes renewable energy.
of the different AGEPAN® Wood Fibreboard products in 2020. Material inherent properties are subject to co­product allocation
Information on the declared unit as ruled in EN 15804.
For the input of post­consumer wood, the carbon stored in
Name Value Unit
wood is inventoried as material inherent property as negative
Declared unit 1 m3 input of stored carbon, expressed in CO ­equivalent, whereas
2
Density 464,2 kg/m³ the energy content of wood is inventoried as input of renewable
secondary material/fuel (as applicable).
The use of secondary wood as a material or fuel input to the
3.2 System boundary product system is inventoried from the end­of­waste status of
Type of the EPD: cradle­to­gate with modules C1 to C4 and the recycled wood onward.
module D (A1­A3, C and D)
Module A4 covers the transport of the product from the
Modules A1 – A3 of the production stage cover the production site to the construction site by a lorry over a default
manufacturing of the products, including raw material extraction distance of 460 km.
and processing, energy generation, the production of ancillary
products and packaging materials, transport, as well as all Module A5 covers the transport of the packaging material from
waste treatment processes. the construction site and its disposal. Default end­of­waste
Eventual benefits of recycling or energy recovery are states for the packaging materials from the packed products at
5 Environmental Product Declaration ­ Sonae Arauco, S.A. ­ AGEPAN® Wood Fibreboards
the construction site are defined in analogy for wastes products were included in the assessment.
occurring in modules A1­A3. Eventual further inputs for the Beyond that, no material or energy flows were neglected that
installation of the products are not considered due to the broad would have been known by the persons re­sponsible for the
applicability of the assessed products. project and that could have been expected to contribute
The substituted primary fuels recovered energy exported from significantly to the environmental indicators declared. It can
the product system in Module A5 are declared in Module D; the thus be assumed that the total contribution of the neglected
benefits of recycled packaging are conservatively neglected processes is not higher than 5 % of the declared impact
due to minimal quantities. categories.
Module C1 manual deconstruction is assumed. 3.5 Background data
The declared values are thus 0. Datasets from ecoinvent 3.7.1 were used as background data
exclusively. Therefore, the latest update of the background data
Module C2 includes the transport of the de­constructed product took place in 2020.
to a recycling centre by over 50 km.
3.6 Data quality
Module C3 covers the preparation of the post­consumer board The requirements on the data quality and the background data
to become a secondary fuel: the end­of­waste status for correspond to the provisions in EN 15804 and the IBU PCR
recycled wood­based boards is defined as the point where they part A (IBU 2020) respectively:
have been sorted and chipped, ready to be used as secondary • Data are as current as possible. Datasets used for
fuels. calculations were updated within the last 10;
• years for generic data and within the last 5 years for
In line with EN 16485, the export of the biogenic carbon stored producer­specific data;
in the board, expressed in CO ­equivalent is also reported in • Datasets are based on 1­year averaged data as a
2
module C3. general rule;
• The time period over which inputs to and outputs from
Module C4 is not relevant for the assumed end­of­life scenario. the system are accounted for is 100 years from the year
The declared values are thus 0. for which the data set is deemed representative;
• The technological coverage reflects the physical reality
Module D compiles all the benefits and burdens associated with of the declared products;
the secondary fuels and exported energy leaving the production • The background datasets comply with the quality
system in the modules A5 and C3. guidelines of ecoinvent 3.7.1; deviations from the
methodological prescriptions of EN 15804 and the IBU
Therefore, module D covers the avoided burdens from energy PCR part A (IBU 2020) respectively are possible but
recovered from the waste treatment in module A5 as well as the acceptable according to IBU PCR part A (IBU 2020).
transports of the obsolete boards to a biomass combustion
3.7 Period under review
plant, the combustion process itself and the loads and benefits
of the substitution of fossil fuels and/or electricity. Substitution The company data gathered for this EPD represents the year
effects in module D are always calculated for the net amount of 2020.
secondary fuel of the product system in line with EN 16485.
3.8 Geographic Representativeness
3.3 Estimates and assumptions Land or region, in which the declared product system is
For the quantification of the net flows of recycled wood (input of manufactured, used or handled at the end of the product´s
post­consumer wood used as a fuel minus post­consumer lifespan: Germany
wood exiting the product system into module D for energy
recovery), it was assumed that all inputs of post­consumer
3.9 Allocation
wood are used as a fuel.
Total fuel input and electricity consumption as well as all
ancillary materials, wastes, airborne emissions and waste water
Beyond that, no relevant estimates or assumptions had to be
on plant level were attributed based on the total weight of the
made beyond the information provided in this EPD.
production volumes of each of the main products produced in
3.4 Cut-off criteria the plant and then broken down to per m3 values.
The applicable criteria for the exclusion of inputs and outputs No separate data were available for the production of the two
are defined in EN 15804, clause 6.3.6, and in the IBU PCR part products. Formaldehyde emissions were attributed 100 % to
A (IBU 2020), respectively. standard MDF production, as the glueing system for AGEPAN®
All data were taken into account that resulted from the data Wood Fibreboard does not contain formaldehyde.
collection procedure in the plant, e.g. related to fuels, raw Consequently, minor amounts of formaldehyde resulting from
material Input, use of ancillary materials, waste flows, the drying of wood in AGEPAN® Wood Fibreboard were
emissions into air, water use, waste water, transport means and attributed to standard MDF.
transport distances, etc. The inventories for the wood inputs were taken from ecoinvent
Expenses for the general management, research & 3.7.1, based on Werner et al. 2015. In these datasets, resource
development, administration and marketing – if known – were corrections are made for incorporated biogenic carbon and
not taken into account. renewable energy; these flows thus reflect the real physical
The production of eventual packaging of ancillary material or flows.
other inputs used during production (and some of the reported Post­consumer secondary wood is used as a fuel input to
wastes) were generally neglected; in most cases reusable bins produce the board; at the input side as well as for the end­of­
or containers are used. In addition, the amounts of reported life scenario, the end­of­waste status was defined after the
(unspecific) wastes are that small that their production can be sorting and chipping of the wood­based board in line with EN
considered not relevant for the life cycle assessment. 16485 (see also clause 3.2). In the end­of­life, loads and
With this approach also mass and energy flows below 1 percent benefits of energy recovery are thus reported in module D.
of total mass and energy flows caused by the declared Waste packaging in module A5 was considered not to reach the
6 Environmental Product Declaration ­ Sonae Arauco, S.A. ­ AGEPAN® Wood Fibreboards
end­of­waste state as a fuel. Its incineration is reported in A5,
the benefits of energy recovery in module D. The benefits of the 3.10 Comparability
recycling of a minor amount of cardboard packaging, steel, and Basically, a comparison or an evaluation of EPD data is only
plastics are disregarded. possible if all the data sets to be compared were created
Biogenic carbon and primary energy content are considered according to EN 15804 and the building context, respectively
material inherent properties and "imported" and "exported" the product­specific characteristics of performance, are taken
to/from the system in line with the mass flows of wood. into account. ecoinvent 3.7.1 has been used as the background
No co­product allocation was made in the modelling of the life database
cycle assessment underlying this EPD.
4. LCA: Scenarios and additional technical information
Characteristic product properties of biogenic carbon Deconstruction (C1)
Manual deconstruction is assumed. The declared values are
Information on describing the biogenic Carbon Content at thus 0.
factory gate
Transport to waste treatment (C2)
Name Value Unit
This module includes the transport of the de­constructed
Biogenic carbon in product 211,3 kg C
product to a recycling centre by a lorry (15% emissions class
Biogenic carbon in packaging 3,87 kg C EURO 5; 85% emissions class EURO 6) by over 50 km.
Waste treatment (C3)
The following technical information is a basis for the declared
464.2 kg of AGEPAN® Wood Fibreboard are chipped and
modules or can be used for developing specific scenarios in the
exported from the product life cycle into module D, assuming a
context of a building assessment if modules are not declared
moisture content of 20% and a lower heating value of 16.6
(MND).
MJ/kg. The biogenic carbon stored in the product and the
content of primary energy are exported from the product system
Transport to the construction site (A4)
as material inherent properties.
The product is transported from the production site to the
construction site by a lorry (15% emissions class EURO 5; 85%
Disposal (C4)
emissions class EURO 6) over a default distance of 460 km.
This module is not relevant for the assumed end­of­life
scenario. The declared values are thus 0.
Installation (A5)
Eventual further inputs for the installation of the products are
Reuse, recycling, recovery potential (D)
not considered due to the broad applicability of the assessed
According to default assumptions in other IBU EPDs, post­
products.
consumer wood is used as a secondary fuel for energy
An average transport distance of 30 km was assumed for
recovery in a biomass combustion plant with an over­all energy
packaging waste from the construction site to the recycling
efficiency of 93% related to the lower heating value of the fuel
plant or to the municipal waste incineration plant. The municipal
input; 91% of the recovered energy is heat, 9% is electricity.
waste incineration plant is assumed to have an overall energy
efficiency of 53% related to the lower heating value of the waste
input; 92% of the recovered energy is heat, 8% is electricity
(according to specifications of MWI plants in ecoinvent 3.7.1).
7 Environmental Product Declaration ­ Sonae Arauco, S.A. ­ AGEPAN® Wood Fibreboards
5. LCA: Results
DESCRIPTION OF THE SYSTEM BOUNDARY (X = INCLUDED IN LCA; ND = MODULE OR INDICATOR NOT DECLARED; MNR =
MODULE NOT RELEVANT)
Benefits and
Construction loads beyond
Product stage Use stage End of life stage
process stage the system
boundaries
la ire ta m w a Ry lp p u s tro p s n a rT g n iru tc a fu n a M e h t m o rf tro p s n a rTe tis e h t o t e ta g y lb m e s s A e s U e c n a n e tn ia M ria p e R tn e m e c a lp e R tn e m h s ib ru fe R y g re n e la n o ita re p Oe s u re ta w la n o ita re p Oe s u n o itc u rts n o c ­e Dn o itilo m e d tro p s n a rT g n is s e c o rp e ts a W la s o p s iD ­e s u e R­y re v o c e R­g n ilc y c e Rla itn e to p
A1 A2 A3 A4 A5 B1 B2 B3 B4 B5 B6 B7 C1 C2 C3 C4 D
X X X X X MND MND MNR MNR MNR MND MND X X X X X
RESULTS OF THE LCA - ENVIRONMENTAL IMPACT according to EN 15804+A2: AGEPAN® Wood Fibreboard, per m³
Parameter Unit A1-A3 A4 A5 C1 C2 C3 C4 D
GWP­total kg CO 2 eq ­4.89E+02 3.7E+01 1.7E+01 0 4.95E+00 7.79E+02 0 ­4.12E+02
GWP­fossil kg CO 2 eq 3E+02 3.7E+01 2.82E+00 0 4.95E+00 3.95E+00 0 ­4.12E+02
GWP­biogenic kg CO 2 eq ­7.89E+02 0 1.42E+01 0 0 7.75E+02 0 0
GWP­luluc kg CO 2 eq 6.8E­01 1.26E­02 5.7E­05 0 2.06E­03 7.99E­03 0 ­1.61E­01
ODP kg CFC11 eq 4.06E­05 8.4E­06 9.24E­08 0 1.09E­06 2.01E­07 0 ­6.01E­05
AP mol H+ eq 1.45E+00 1.1E­01 5.44E­03 0 1.45E­02 2.1E­02 0 ­4.65E­01
EP­freshwater kg P eq 2.49E­02 2.76E­04 2.39E­06 0 4.25E­05 4.09E­04 0 ­8.02E­03
EP­marine kg N eq 4.49E­01 2.46E­02 2.47E­03 0 3.13E­03 2.88E­03 0 ­3.46E­02
EP­terrestrial mol N eq 4.21E+00 2.73E­01 2.77E­02 0 3.48E­02 3.27E­02 0 ­3.84E­01
kg NMVOC
POCP 2.46E+00 9.86E­02 8.18E­03 0 1.26E­02 9.09E­03 0 ­2E­01
eq
ADPE kg Sb eq 1.91E­03 1.35E­04 6.53E­07 0 2.35E­05 9.82E­06 0 ­1.88E­04
ADPF MJ 5.46E+03 5.6E+02 6.05E+00 0 7.41E+01 8.1E+01 0 ­7.94E+03
m3 world eq
WDP 1.04E+02 1.62E+00 3.26E­02 0 2.33E­01 8.44E­01 0 ­1.4E+01
deprived
GWP = Global warming potential; ODP = Depletion potential of the stratospheric ozone layer; AP = Acidification potential of land and water; EP =
Eutrophication potential; POCP = Formation potential of tropospheric ozone photochemical oxidants; ADPE = Abiotic depletion potential for non­fossil
resources; ADPF = Abiotic depletion potential for fossil resources; WDP = Water (user) deprivation potential)
RESULTS OF THE LCA - INDICATORS TO DESCRIBE RESOURCE USE according to EN 15804+A2: AGEPAN® Wood
Fibreboard, per m³
Parameter Unit A1-A3 A4 A5 C1 C2 C3 C4 D
PERE MJ 1.47E+02 7.5E+00 1.39E+02 0 1.17E+00 1.25E+01 0 ­2.52E+02
PERM MJ 8.17E+03 0 ­1.39E+02 0 0 ­8.03E+03 0 0
PERT MJ 8.31E+03 7.5E+00 6.65E­02 0 1.17E+00 ­8.01E+03 0 ­2.52E+02
PENRE MJ 4.65E+03 5.61E+02 5.53E+01 0 7.42E+01 8.84E+02 0 ­7.85E+03
PENRM MJ 8.51E+02 0 ­4.92E+01 0 0 ­8.02E+02 0 0
PENRT MJ 5.5E+03 5.61E+02 6.05E+00 0 7.42E+01 8.17E+01 0 ­7.85E+03
SM kg 3.1E­01 0 0 0 0 0 0 0
RSF MJ 3.57E+02 0 0 0 0 0 0 7.67E+03
NRSF MJ 0 0 0 0 0 0 0 8.02E+02
FW m3 9.61E+00 3.43E­01 1.34E­03 0 1.34E­03 1.4E+00 0 ­2.83E+01
PERE = Use of renewable primary energy excluding renewable primary energy resources used as raw materials; PERM = Use of renewable primary
energy resources used as raw materials; PERT = Total use of renewable primary energy resources; PENRE = Use of non­renewable primary energy
excluding non­renewable primary energy resources used as raw materials; PENRM = Use of non­renewable primary energy resources used as raw
materials; PENRT = Total use of non­renewable primary energy resources; SM = Use of secondary material; RSF = Use of renewable secondary fuels;
NRSF = Use of non­renewable secondary fuels; FW = Use of net fresh water
RESULTS OF THE LCA – WASTE CATEGORIES AND OUTPUT FLOWS according to EN 15804+A2:
AGEPAN® Wood Fibreboard, per m³
Parameter Unit A1-A3 A4 A5 C1 C2 C3 C4 D
HWD kg 5.23E­03 1.46E­03 5.57E­06 0 1.98E­04 3.25E­05 0 ­8.4E­03
NHWD kg 4.25E+01 2.74E+01 1.68E­01 0 2.95E+00 5.07E­01 0 1.31E+00
RWD kg 3.07E­02 8.21E­03 8.23E­05 0 1.07E­03 1.04E­03 0 ­2.61E­02
CRU kg 0 0 0 0 0 0 0 0
MFR kg 3.38E­01 0 9.38E­01 0 0 0 0 0
MER kg 0 0 0 0 0 4.64E+02 0 0
EEE MJ 3.37E­02 0 6.91E+00 0 0 0 0 0
EET MJ 3.87E­01 0 7.95E+01 0 0 0 0 0
8 Environmental Product Declaration ­ Sonae Arauco, S.A. ­ AGEPAN® Wood Fibreboards
HWD = Hazardous waste disposed; NHWD = Non­hazardous waste disposed; RWD = Radioactive waste disposed; CRU = Components for re­use;
MFR = Materials for recycling; MER = Materials for energy recovery; EEE = Exported electrical energy; EET = Exported thermal energy
RESULTS OF THE LCA – additional impact categories according to EN 15804+A2-optional:
AGEPAN® Wood Fibreboard, per m³
Parameter Unit A1-A3 A4 A5 C1 C2 C3 C4 D
Disease
PM 1.04E­05 2.36E­06 7.51E­08 0 2.71E­07 6.05E­08 0 ­3.11E­07
incidence
IR kBq U235 eq 1.37E+01 2.46E+00 2.43E­02 0 3.27E­01 7.04E­01 0 ­1.52E+01
ETP­fw CTUe 9.45E+03 4.3E+02 5E+00 0 5.92E+01 4.53E+01 0 ­7.8E+02
HTP­c CTUh 1.82E­06 1.53E­08 2.86E­09 0 2.35E­09 2.71E­09 0 1.04E­07
HTP­nc CTUh 1.7E­05 4.22E­07 1.17E­08 0 5.49E­08 3.6E­08 0 ­3.07E­07
SQP SQP 4.76E+04 3.91E+02 1.22E+00 0 4.4E+01 1.19E+01 0 ­2.55E+02
PM = Potential incidence of disease due to PM emissions; IR = Potential Human exposure efficiency relative to U235; ETP­fw = Potential comparative
Toxic Unit for ecosystems; HTP­c = Potential comparative Toxic Unit for humans (cancerogenic); HTP­nc = Potential comparative Toxic Unit for humans
(not cancerogenic); SQP = Potential soil quality index
Disclaimer 1 – for the indicator “Potential Human exposure efficiency relative to U235”.This impact category deals mainly with the
eventual impact of low dose ionizing radiation on human health of the nuclear fuel cycle. It does not consider effects due to possible
nuclear accidents, occupational exposure or due to radioactive waste disposal in underground facilities. Potential ionizing radiation
from the soil, radon and from some construction materials is also not measured by this indicator.
Disclaimer 2 – for the indicators “abiotic depletion potential for non­fossil resources”, “abiotic depletion potential for fossil resources”,
“water (user) deprivation potential, deprivation­weighted water consumption”, “potential comparative toxic unit for ecosystems”,
“potential comparative toxic unit for humans – cancerogenic”, “Potential comparative toxic unit for humans ­ not cancerogenic”,
“potential soil quality index”. The results of this environmental impact indicator shall be used with care as theuncertainties on these
results are high as there is limited experience with the indicator.
6. LCA: Interpretation
The following Figure illustrates the contribution of each life assessment (impact from module A1­C4 = 100 %).
cycle stage to the overall indicator results of the impact
are not significant.
Figure 1: Environmental impacts of AGEPAN® Wood It illustrates also that for the GWP, the ODP and the ADP fossil,
Fibreboard along its life cycle (impacts from production the benefits from the energy recovery of AGEPAN® Wood
modules A1-C4 = 100) Fibreboard are higher than the impacts during the life cycle,
notably the impacts from production; for other impact
Figure 1 shows that the impacts over the life cycle of the categories, the benefits of energy recovery lie between 10 % to
product are predominantly caused during the production of the 35 %, depending on the impact category under consideration.
wood fibreboard; the impacts from other parts of the life cycle
9 Environmental Product Declaration ­ Sonae Arauco, S.A. ­ AGEPAN® Wood Fibreboards
The global warming potential (GWP) is an indicator for the combustion processes or disposal processes, e.g., of mining
contribution to climate change and is quan­tified based on the residues from lignite extraction related to the generation of
emissions of gases that absorb radiative forcing. electricity.
The EP is caused mainly by airborne emissions of nitrogen
The production phase of AGEPAN® Wood Fibreboard is largely oxides as well as phosphate emissions into the groundwater.
caused by the upstream processes of the production of PMDI
(around 30 %); the generation of electricity causes around 35% The photochemical oxidation potential (POCP) assesses the
of the GWP, the use of natural gas during production causes contribution of airborne emissions that contribute to summer
another 20 %; in sum, 10 % of the GWP are related to the ozone creation.
forestry processes and by the transport for raw material About 65% of the POCP are caused by the on­site emissions at
acquisition. the production site. 20 % of the POCP are associated with the
production of PMDI resins; another 8% are caused by
Figure 2 illustrates that the biogenic carbon stored in the harvesting operations of stemwood and its transport to the
product, expressed as CO ­equivalent, is higher than the CO production site.
2 2
These contributions are caused by emissions of SO , CO and
emissions from fossil sources, leading to a negative GWP for 2
the production mod­ule A1­A3. The potential substitution effect CH 4.
in module D more than offsets the GHG emissions during the
production phase (module A1­A3). The abiotic resource depletion potential of fossil resources
(ADP fossil) assesses the use of scarce fossil resources such
The GWP is dominated by CO 2 emissions and removals. as natural gas or crude oil.
The ADP (fossil resources) is caused mainly by the production
of PMDI (35%), by the on­site consumption of natural gas
(20%) and by the generation of electricity (30%).
The abiotic resource depletion potential for mineral resource
(ADP elements) assesses the use of scarce mineral resources
such as ores and other mineral raw materials.
The ADP (elements) is caused almost completely by
infrastructure processes, such as the buildings required for the
production of chemicals; the main resources contributing to the
ADP (elements) are copper, zinc and gold.
Selected indicators from the life cycle inventory
The main use of renewable primary energy is the heating value
of the wood in AGEPAN® Wood Fibreboard; this amount of
non­used renewable energy is exported in module C3 and used
Figure2: Carbon footprint of AGEPAN®Wood Fibreboard
energetically as a renewable secondary fuel in module D. The
renewable primary energy used as energy is mainly woody
The ozone layer depletion potential (ODP) is quantified based
biomass.
on the emissions of gases that can de­stroy stratospheric
ozone.
The major share of the non­renewable primary energy is used
energetically, mainly as natural gas in the upstream processes
The ODP is caused mainly by emissions of Halon 1211, which
for the production of PMDI. A minor share is used as a material,
are associated with the production and transport of natural gas.
i.e., as com­po­nents of the gluing systems; this non­renewable
Around 20 % of the ODP are associated with the use of natural
primary energy used as a material is not used within the life
gas on­site for the production of AGEPAN® Wood Fibreboard,
cycle of AGEPAN® Wood Fiberboard; it is exported in module
the rest of the ODP is caused by the use of natural gas in
C3 and used energetically as a non­renewable secondary fuel
upstream processes in line with the consumption patterns of
in module D.
natural gas in the process chain, notably for the production of
The indicator values for wastes refer to the amount of wastes
PMDI.
that is landfilled after an eventual pre­treatment of the wastes.
The acidification potential (AP) is created with the
The main part of the wastes associated with the production of
transformation of airborne emissions into acids, which among
other can reduce soil fertility. AGEPAN® Wood Fibreboard is non­hazardous waste, mainly
resulting from the disposal of the infrastructure associated with,
Roughly, 25% of the AP are caused by the on­site combustion e.g., production halls or roads.
processes for the production of heat; the other 75 % are Hazardous wastes are generated throughout the production
associated with upstream combustion processes, notably for chain, e.g., related to the disposal of ashes, production wastes
heat production in the production of the PMDI (50 %), for the from chemical industry or from the production of primary
generation of electricity (17 %), and related to production and aluminium for infrastruc­ture processes.
transport of wood inputs (10%). The generation of radioactive waste is associated with the
production of nuclear power.
The AP is caused in comparable shares by emissions of
ammonia, nitrogen oxides and sulphur dioxide. The net consumption of fresh water is caused mainly by cooling
processes throughout the production chain as well as partly by
The eutrophication potentials (EP) quantify the accumulation of the generation of electricity.
nutrients in soils and watersheds, which can cause increased
growth of algae and shifts in species composition. The further indicators on environmental aspects are singular
The EP is caused by a variety of processes, mainly in values that result from the inventorying of waste streams into
10 Environmental Product Declaration ­ Sonae Arauco, S.A. ­ AGEPAN® Wood Fibreboards
thermal waste treatment, energy recovery and recycling.
7. Requisite evidence
Measuring agency: Eurofins Denmark
7.1. Formaldehyde
Test report, date: G11664 and G15792, dated 17­01­2012 and
AGEPAN® Wood Fibreboards meet the requirements of the 19­06­2012
German Chemicals Prohibition Regulation (ChemVerbotsV),
Result: The measured emissions were lower than 1000 μg/m3,
ZE05 Certificates by MPA Eberswalde, No. resulting in a classification A+.
31/22/3757/01/ZE05 The determination of the formaldehyde AGEPAN® fiberboards are labelled as class A according to the
content according to DIN EN 717­1 (chamber method) for French regulation on the labelling of emissions of volatile
AGEPAN® Wood Fibreboards are below 0.05 ppm, complying pollutants (with reference to the wall scenario, as a worst case).
with the E1 requirements of EN13986.
Measuring agency: MPA Eberswalde
Measuring agency: MPA Eberswalde
Product, test reports, date:
Test report, date: 31/21/4562/01, dated 02­12­2021 THD, 31/18/3359/03, 04.05.2018 UDP, 31/18/3359/01,
04.05.2018 DWD, 31/18/3359/02, 04.05.2018
Result: Formaldehyde emissions tests were performed for AgBB overview of results (28 days [µg/m³])
DWD and values measured was 0,012 ppm (below the 0,05
Name Value Unit
ppm limit) 7.2. MDI
TVOC (C6 ­ C16) 0,7 μg/m3
For PMDI­bonded boards: Sum SVOC (C16 ­ C22) < 0,005 μg/m3
Measuring agency: Wessling Beratende Ingenieure GmbH,
R (dimensionless) 1 ­
Altenberg, Germany
VOC without NIK < 0,005 μg/m3
Test report, date: IAL­09­0566 dated 12 January 2010 Carcinogenic Substances < 1 μg/m3
7.5 PCP/Lindane
Result: Test chamber analysis of wooden materials (MDI). The
analysis was carried out in accordance with the test guidelines
The wood preservative agents pentachlorophenol (PCP) and
of the RAL Environmental Label 76 (wooden materials). No lindane are not detected in the AGEPAN® fiberboards
emissions of monomer MDI and other isocyanates in the test
chamber could be detected. The detection limit was 0.1µg/m3.
Measuring agency: MPA Eberswalde, Materialprüfanstalt
7.3 Checking for the pre-treatment of the substances used
Brandenburg GmbH, Germany
No post­consumer wood is used in the production of AGEPAN®
Wood Fibreboard. . 7.4 TVOC emissions Test report, date: 31/21/4562/01, dated 02­12­2021
VOC emissions tests were performed for THD and DWD Result: PCP and lindane could not be determined in the board
products according to ISO16000-11, with the wall panel loading sample of AGEPAN® DWD, examined. Limit of determination:
scenario.
0.10 mg/kg.
8. References
Product category rules of IBU Environmental product declarations ­ Core rules for the product
category construction products.
IBU (2021)
IBU (2021): General Instructions for the EPD Programme of the ISO 14025
Institut Bauen & Umwelt e.V. (General Instructions for the IBU ISO 14025:2006­07, Environmental labels and declarations ­
EPD Programme). Version 2.0, Institut Bauen & Umwelt, Berlin. Type III Environmental declarations ­ Principles and
procedures.
IBU (2021)
IBU (2021): PCR Part A: Calculation rules for the life cycle ISO 14044
assessment and requirements for the project report according EN ISO 14044:2006­07, Environmental management ­ Life
to EN 15804+A2:2019. Version 2.1., Institut Bauen & Umwelt, cycle assessment ­ Requirements and guidance (ISO
Berlin. 14044:2006); German and English versions EN ISO
14044:2006.
IBU (2019)
Institut Bauen und Umwelt e.V, Berlin (pub.): Product Category ISO 9001
Rules for Construction Products from the range of ISO 9001:2015, Quality management systems – Requirements.
Environmental Product Declarations for Institut Bauen und
Umwelt (IBU), Part B: Requirements on the EPD of wood based ISO 14001
panels, 2019­01. ISO 14001:2015, Environmental management systems –
Requirements with guidance for use.
Standards and legal documents
EN 15804 OHSAS 18001
EN 15804+A2:2019, Sustainability of construction works ­ OHSAS 18001:2007, Occupational Health and Safety
11 Environmental Product Declaration ­ Sonae Arauco, S.A. ­ AGEPAN® Wood Fibreboards
Management Systems – Requirements. EN ISO 50001
EN ISO 50001:2018­12, Energy management systems –
ISO 45001 Requirements with guidance for use.
ISO 45001:2018:03, Occupational health and safety
management systems ­ Requirements with guidance for use. Regulation (EU) No. 305/2011
Regulation No. 305/2011 (Construction Products Regulation, or
ISO 16000 CPR) of the European Parliament and of the European Council
ISO 16000­11:2006, Indoor air – Part 11: Determination of the is a regulation of 9 March 2011 that lays down harmonised
emission of volatile organic compounds from building products conditions for the marketing of construction products and
and furnishing – Sampling, storage of samples and preparation replaces Construction Products Directive (89/106/EEC).
of test specimens.
ECHA candidate list
EN 717-1 Candidate List of substances of very high concern for
EN 717­1:2005­01, Wood­based panels – Determination of Authorisation, published in accordance with Article 59(10) of the
formaldehyde release – Formaldehyde emission by the REACH Regulation. European Chemicals Agency, Brussels.
chamber method.
Ordinance on Biocide Products No. 528/2012
EN 13501 REGULATION (EU) No 528/2012 OF THE EUROPEAN
EN 13501­1:2019­05, Fire classification of construction PARLIAMENT AND OF THE COUNCIL of 22 May 2012
products and building elements – Classification using test data concerning the making available on the market and use of
from reaction to fire tests. biocidal products.
EN 13171 European List of Waste
EN 13171:2008, Thermal insulation products for buildings – Commission Decision of 3 May 2000 replacing Decision
Factory made wood fibre (WF) products – Specification. 94/3/EC establishing a list of wastes pursuant to Article 1(a) of
Council Directive 75/442/EEC on waste and Council Decision
EN 14964 94/904/EC establishing a list of hazardous waste pursuant to
EN 14964: 2007­01, Rigid underlays for discontinuous roofing ­ Article 1(4) of Council Directive 91/689/EEC on hazardous
Definitions and characteristics. waste (notified under document number C(2000) 1147).
DIN 4108 Additional references
DIN 4108, Thermal protection and energy economy in buildings
(several parts). ecoinvent 3.7.1
Life cycle inventory data, December 2020. Ecoinvent Center,
EN 300 Zurich.
EN 300: 2006, Oriented Strand Boards (OSB) – Definitions,
classification and specifications. Werner et al. 2015
Werner F., Bauer C., Büsser S., Doka G., Kaufmann E., Kono
EN 16485 J., Luginbühl, U., Mina M., Frischknecht R., Thees O, Wallbaum
EN 16485:14­07, Round and sawn timber – Environmental H., Zimmermann W., Hischier R. (2014): Aktualisierung der
Product Declarations – Product category rules for wood and Modelle und Datensätze zu Holz und Holzprodukten in der
wood­based products for use in construction. Datenbank ecoinvent. Commissioner: Bundesamt für Umwelt,
Aktionsplan Holz, Bern. Final report 18. February 2015.
12 Environmental Product Declaration ­ Sonae Arauco, S.A. ­ AGEPAN® Wood Fibreboards
Publisher
Institut Bauen und Umwelt e.V. +49 (0)30 3087748­ 0
Hegelplatz 1 info@ibu­epd.com
10117 Berlin www.ibu­epd.com
Germany
Programme holder
Institut Bauen und Umwelt e.V. +49 (0)30 3087748­ 0
Hegelplatz 1 info@ibu­epd.com
10117 Berlin www.ibu­epd.com
Germany
Author of the Life Cycle Assessment
Dr. Frank Werner ­ Umwelt & Entwicklung + 41 (0)44 241 39 06
Idaplatz 3 frank@frankwerner.ch
8003 Zürich http://www.frankwerner.ch/
Switzerland
Owner of the Declaration
Sonae Arauco, S.A. (+34) 918 070 701
Centro Empresarial Euronova, C/Ronda de products@sonaearauco.com
Poniente, 6 ­ B www.sonaearauco.com
28760 Tres Cantos (Madrid)
Spain
Sonae Arauco Deuschland GmbH +49 (0) 5391 405 316
Grecostraße 1 info.agepan@sonaearauco.com
49716 Meppen www.sonaearauco.com
Germany
13 Environmental Product Declaration ­ Sonae Arauco, S.A. ­ AGEPAN® Wood Fibreboards
