ENVIRONMENTAL PRODUCT DECLARATION
as per ISO 14025 and EN 15804+A2
Owner of the Declaration Etex Building Performance International
Publisher Institut Bauen und Umwelt e.V. (IBU)
Programme holder Institut Bauen und Umwelt e.V. (IBU)
Declaration number EPD-ETE-20240005-IBC1-EN
Issue date 12.03.2024
Valid to 11.03.2029
PregyMetal AquaBoard - AZ150 galvanized steel profiles with
0,6mm thickness
Etex Building Performance SpA
www.ibu-epd.com | https://epd-online.com
1. General Information
Etex Building Performance SpA PregyMetal AquaBoard - AZ150 galvanized steel
profiles with 0,6mm thickness
Programme holder Owner of the declaration
IBU – Institut Bauen und Umwelt e.V. Etex Building Performance International
Hegelplatz 1 Rue Marcel Demonque 500
10117 Berlin 84915 Avignon Cedex 9
Germany France
Declaration number Declared product / declared unit
EPD-ETE-20240005-IBC1-EN 1 kg of average steel structure for PregyMetal "AquaBoard" profile with
0,6mm thickness.
This declaration is based on the product category rules: Scope:
Structural steels, 01.08.2021 This EPD is an average EDP and applies for the following specific SINIAT
(PCR checked and approved by the SVR) produts brand developed by Etex Builfding Performace S.p.A: Montante
PregyMetal AquaBoard C50/50 (or Montante PregyMetal XT C50/50),
Montante PregyMetal AquaBoard C75/50 (or Montante PregyMetal XT
Issue date C75/50), Montante PregyMetal AquaBoard C100/50 (or Montante
PregyMetal XT C100/50), Montante PregyMetal AquaBoard C150/50 (or
12.03.2024
Montante PregyMetal XT C150/50), Profilo PregyMetal AquaBoard S6027
BA, Guida PregyMetal AquaBoard U50/40 (or Guida PregyMetal XT
U50/40), Guida PregyMetal AquaBoard U75/40 (or Guida PregyMetal XT
Valid to
U75/40), Guida PregyMetal AquaBoard U100/40 (or Guida PregyMetal XT
11.03.2029 U100/40), Guida PregyMetal AquaBoard U150/40 (or Guida PregyMetal
XT U150/40), Guida PregyMetal AquaBoard U28/28 (or Guida PregyMetal
XT U28/28), Profilo PregyMetal Aquaboard S6027 BA (or Profilo
Pregymetal XT S6027 BA)
This EPD was developed from data collected at the Etex Building
Performace S.p.Asteel profile factory located in Corfinio. CAP 67030 (AQ),
Italy, producing 100% of the total production of these products. Data refers
to year 2021.
The EPD is a cradle-to-gate with options EPD and covers Siniat
PregyMetal AquaBoard steel profiles.
Dipl.-Ing. Hans Peters
The owner of the declaration shall be liable for the underlying information
(Chairman of Institut Bauen und Umwelt e.V.)
and evidence; the IBU shall not be liable with respect to manufacturer
information, life cycle assessment data and evidences.
The EPD was created according to the specifications of EN 15804+A2. In
the following, the standard will be simplified as EN 15804.
Verification
The standard EN 15804 serves as the core PCR
Independent verification of the declaration and data according to ISO
14025:2011
internally X externally
Florian Pronold Vito D'Incognito,
(Managing Director Institut Bauen und Umwelt e.V.) (Independent verifier)
1 Environmental Product Declaration - Etex Building Performance SpA - PregyMetal AquaBoard - AZ150 galvanized steel profiles with 0,6mm thickness
2. Product
Name Value Unit
2.1 Product description/Product definition
Density 7.85 kg/m3
Siniat PregyMetal AquaBoard profiles covered by this EPD are
used in the construction sector as a support framing for Guida PregyMetal AquaBoard U100/40 or Guida 1.24 m
plasterboard walls and ceilings. Three main groups can be PregyMetal XT U100/40
distinguished: Guida PregyMetal AquaBoard U150/40 or Guida
0.98 m
- 'U' tracks Guide, profiles that, on the floor and ceiling, block PregyMetal XT U150/40
the foot and head of the vertical studs of the wall warps, Guida PregyMetal AquaBoard U28/28 or Guida
2.85 m
- 'C' studs Montanti, profiles that constitute the vertical PregyMetal XT U28/28
structures of the wall frames,
Guida PregyMetal AquaBoard U50/40 or Guida
- 'C' channels Profili, profiles used to form the frame for a 1.8 m
PregyMetal XT U50/40
suspended ceiling system.
Guida PregyMetal AquaBoard U75/40 or Guida
The galvanized carbon steel profiles here studied have a 1.5 m
PregyMetal XT U75/40
AZ150 aluminum and zinc coating (150 g/m2 as minimum
Montante PregyMetal AquaBoard C100/50 or
weight), mainly used for external walls and ceilings or internal 1.07 m
Montante PregyMetal XT C100/50
high humidity areas.
The EPD covers the Italian version of the steel profiles for Montante PregyMetal AquaBoard C150/50 or
0.82 m
plasterboards drywall system. Montante PregyMetal XT C150/50
The EPD refers to 1 average kg of steel profiles with coating. Montante PregyMetal AquaBoard C50/50 or
1.4 m
For the placing on the market of the product in the European Montante PregyMetal XT C50/50
Union/European Free Trade Association (EU/EFTA) (with the Montante PregyMetal AquaBoard C75/50 or
exception of Switzerland) Regulation (EU) No. 305/2011 (CPR) Montante PregyMetal XT C75/50 1.2 m
applies. The product needs a declaration of performance taking
Profilo PregyMetal AquaBoard S6027 BA or
into consideration EN 14195:2005, Metal framing components 1.89 m
Profilo Pregymetal XT S6027 BA
for gypsum board systems - Definitions, requirements and test
methods and the CE-marking. Performance data of the product in accordance with the
For the application and use the respective national provisions declaration of performance with respect to its essential
apply. characteristics according to UNI EN 14195:2005
2.2 Application 2.4 Delivery status
Siniat PregyMetal profiles covered by this EPD are used in all Siniat PregyMetal AquaBoard profiles covered by this EPD are
construction types (residential, commercial, healthcare, ...new delivered in variable dimensions, specified by their respective
or renovation), to build drywall systems. The various profiles data sheets available at www.siniat.it. The typical length of the
can be used as vertical plasterboard frames, with improved structures is 3 m. The selling unit is a set of a defined number
stiffness and mechanical properties for high walls. They can be of structures bound by different plastic straps and separated by
considered easy to install products. wooden slats.
Possible plasterboard frames fields of application are:
2.5 Base materials/Ancillary materials
- Interior use, for walls and ceilings,
- Exterior use, for facade, sheathing walls, ceilings and eaves. Steel structure
Name Value Unit
2.3 Technical Data
Detailed technical information is available in the specific Galvanized carbon steel DX51D 1 Kg
product data sheets at www.siniat.it. Recycled steel content 35 %
Siniat PregyMetal AquaBoard profiles covered by this EPD are
- Performance data of the product in accordance with the
made from galvanized carbon steel DX51D with 35% of post
declaration of performance with respect to its essential
consumer recycled content.
characteristics according to UNI EN 14195:2005
The metallic coating is the AZ150 Aluzinc coating is
- Tensile strenght: ≥ 300 N/mm2
represented of 55% aluminium, 43,4% zinc and 1,6% silicon.
The steel profiles covered by this EPD do not contain any
- Quality steel grade: DX51 D+AZ150
substances listed in the 'Candidate List of Substances of Very
High Concern for Authorisation' (SVHC)
- Class of reaction to fire performance: A1
/(https://echa.europa.eu/it/candidate-list-table - date:
Constructional data 27.06.2018)/ exceeding 0.1% by mass.
Below is a list of the number of meters necessary to obtain 1 kg
of each individual product (o profile) The Candidate list can be found on the ECHA website address:
https://echa.europa.eu/de/home.
The steel structures covered by this EPD do not contain any
other carcinogenic, mutagenic, reprotoxic (CMR) substances in
categories 1A or 1B which are not on the candidate list,
exceeding 0.1% by mass.
2.6 Manufacture
The manufacturing process is illustrated in the Figure below.
The production process consists of cutting, modeling, and
2 Environmental Product Declaration - Etex Building Performance SpA - PregyMetal AquaBoard - AZ150 galvanized steel profiles with 0,6mm thickness
drilling of channels, studs and metal tracks. The raw materials life. The material composition of the product does not change
first arrive at the plants in the form of rolls of galvanized steel, during its use phase.
separated from each other by wooden slats, bound by plastic
straps and subsequently stored inside the Company's 2.11 Environment and health during use
warehouse. The actual process begins when the rolls of raw These products are not classified as hazardous under the EU
material are placed at the beginning of special machines that CLP Regulation (European Regulation EC/1272/2008 on the
work the profiles. Initially, the steel coil is unrolled and passes classification, labelling and packaging of substances and
through a set of rollers that gives the desired shape (U or C). mixtures).
Subsequently, the profile thus formed passes through a
2.12 Reference service life
machine that drills it according to pre-established schemes.
Finally, the formed and perforated steel structures are cut in The reference service life (RSL) is not relevant for
length according to predetermined measures. The finished consideration of the LCA as the steel structures are long-lasting
products are then grouped and held together by plastic products, therefore the use phase is not considered.
strapping and separated from each other with wooden slats. Furthermore, the use stage (modules B1-B7) doesn't cause any
The management system operated by the site is in compliance environmental impact as the structures, once installed, do not
with the UNI EN ISO 9001:2015. require any manufacturing, water or electricity use or
substitutions. In this particular case, in accordance with the
"Federal office for building an regional planning" BBSR table
"Service lives of components for life cycle assessment
according to BNB" (http://www.nachhaltigesbauen.de/baustoff-
und-gebaeudedaten/nutzungsdauern-von-bauteilen.html), a
service life can be declared (not a RSL according to ISO
15686). The voice 'Unterkonstruktionen: Trockenbauprofile
(Stahl, Holz)', meaning Drywall profiles for substructures, here
in steel. The service life is considered to be higher than 50
years.
Description of the influences on the ageing of the product when
applied in accordance with the rules of technology.
2.7 Environment and health during manufacturing 2.13 Extraordinary effects
Relating to health protection during the manufacturing process, Fire
the plant follows and respects the specific Italian Regulation. Information on the fire performance according to EN 13501:1 or
The manufacturing process is certified according to established national standards. According to EN 13501:1:
Occupational Health and Safety Management System UNI ISO
45001:2018.
Steel profiles are manufactured in a plant permitted by emission - The classes of building products regarding their fire
law and by external waste recovery in accordance with the performance are predefined as: A1
Italian regulation. The management system operated by the site Water
is in compliance with the standard UNI EN ISO 14001:2015. Contains no substances that have any impact on water in case
of flood.
2.8 Product processing/Installation
The manufacturing process is carried out in dedicated Mechanical destruction
automated machines that work the profiles: security protections If relevant: information on the product performance including
according to the safety machinery standards are installed to possible impacts on the environment following unforeseeable
avoid any risks for operators. mechanical destruction.
During handling, storage and installation: eye protection should
be worn when using hand tools, gloves should be worn when
2.14 Re-use phase
handling metal sections and components to avoid risk of
lacerations, packs should be stacked in a safe and stable For the "C3" recycling phase, a scenario was used that
manner, pack strapping should not be used for lifting, coils and recovers 90% of the steel and therefore sent for material
metal sections may spring apart when strapping is released. recovery
2.9 Packaging 2.15 Disposal
For product protection the steel profiles are packed in groups of Disposal in accordance with the waste code: 17 04 05 Steel
192 or 360 and held together with plastic strapping and wooden and iron waste from construction and demolition operations.
slats. The structures can be dissembled and, since they are entirely
made out of steel, at least 90% can be recycled.
2.10 Condition of use National disposal guidelines have to be observed.
Siniat PregyMetal AquaBoard profiles for plasterboard are
2.16 Further information
suitable for any type of wall and ceiling created for plasterboard
systems. No maintenance or repair is required over the service www.siniat.it
3. LCA: Calculation rules
Declared unit and mass reference
3.1 Declared Unit
The LCA results presented in this EPD are related to 1 kg of
average steel profile with 0,6mm thickness. The arithmetic
mean was carried out between the environmental impact
results of the different products considered.
3 Environmental Product Declaration - Etex Building Performance SpA - PregyMetal AquaBoard - AZ150 galvanized steel profiles with 0,6mm thickness
Name Value Unit
3.3 Estimates and assumptions
Declared unit 1 kg
Assumptions regarding transport distances were made for the
Conversion factor:
installation and end-of-life of the studied products, following the
Guida PregyMetal AquaBoard U100/40 or Guida indications found in the EN 15804+A2 standard.
1.24 m/kg
PregyMetal XT U100/40
3.4 Cut-off criteria
Guida PregyMetal AquaBoard U150/40 or Guida
0.98 m/kg
PregyMetal XT U150/40 In this study the packaging relating to the packaging materials
of the finished product were placed in Cut-Off
Guida PregyMetal AquaBoard U28/28 or Guida
2.85 m/kg
PregyMetal XT U28/28
3.5 Background data
Guida PregyMetal AquaBoard U50/40 or Guida
1.8 m/kg The life cycle model supporting the EPD was developed in
PregyMetal XT U50/40
SimaPro 9.5, using background data from Ecoinvent 3.9.1, with
Guida PregyMetal AquaBoard U75/40 or Guida the cutoff system model. When background data representative
1.5 m/kg
PregyMetal XT U75/40 of the Italian market was not available in the Ecoinvent
Montante PregyMetal AquaBoard C100/50 or database, European average data ('Europe without Switzerland'
1.07 m/kg
Montante PregyMetal XT C100/50 or 'RER') or global data ('GLO') was used instead.
Montante PregyMetal AquaBoard C150/50 or
0.82 m/kg 3.6 Data quality
Montante PregyMetal XT C150/50
Background data is from the Ecoinvent 3.9.1 database. Some
Montante PregyMetal AquaBoard C50/50 or
1.4 m/kg of these background datasets have been collected more than
Montante PregyMetal XT C50/50
10 years ago but are still representative of current technology.
Montante PregyMetal AquaBoard C75/50 or 1.2 m/kg Primary data provided by Etex Building Performace S.p.A and
Montante PregyMetal XT C75/50 reviewed by Greenwich Srl is representative of the annual
Profilo PregyMetal AquaBoard S6027 BA or production for the year 2021.Since this is an average EPD, the
1.89 m/kg
Profilo Pregymetal XT S6027 BA environmental impacts reported are considered representative
Density 7500 kg/m3 of all products as both the raw material and the production
process remain identical.
3.2 System boundary 3.7 Period under review
This EPD is a cradle-to-gate with options EPD, covering the The data used for the study complies with the current level of
following life cycle stages: knowledge at the time of modelling the LCA in 2021.
3.8 Geographic Representativeness
• steel structures manufacturing (modules A1-A3),
including the production of the steel rolls, the transport Land or region, in which the declared product system is
to the manufacturing site, as well as impacts due to manufactured, used or handled at the end of the product´s
energy consumption, as well as auxiliary materials, lifespan: EU-27 Member States
waste treatment;
• transport of the steel structures from the manufacturing
3.9 Allocation
to the building site (module A4),
In accordance with the PCR, the allocation was made
Installation (module A5), including the production of
considering the production of 2021. Specifically, the total
auxiliaries and of waste deriving from packaging;
quantity of profiles produced at the Corfinio plant, measured in
• emissions during the use phase (modules B). No
mass (kg), was obtained from the internal monitoring reports.
emissions occur during the Etex Building Performace
The percentage of the studied metal structures compared to the
S.p.A steel structure use phase;
total production within the Corfinio plant is 91%.
• end-of-life (modules C1-C4), including impacts from
manual deconstruction, transport of waste to treatment
3.10 Comparability
facility, and waste processing and waste disposal. The
Basically, a comparison or an evaluation of EPD data is only
scenario studied considers 90% of the structure
possible if all the data sets to be compared were created
recyclable (C3) and 10% sent to landfill (C4);
according to EN 15804 and the building context, respectively
• benefits and loads beyond the system boundaries (D).
the product-specific characteristics of performance, are taken
into account. Background data base : Ecoinvent 3.9.1
4. LCA: Scenarios and additional technical information
Installation into the building (A5)
Characteristic product properties of biogenic carbon
For the installation phase, a typical situation was estimated per
The total mass of biogenic carbon containing materials is less
meter of structure installed:
than 5 % of the total mass of the product and accompanying
- screws per meter = 10
packaging.Note: 1 kg of biogenic carbon is equivalent to 44/12
- seconds needed to tighten a screw = 5
kg of CO2.
- Total operating time = 50 seconds
- Drill power = 600 W
The A5 installation phase considers all materials, waste and
A consumption of 0.0208 kWh of electricity is therefore
energy consumed to install the studied product at the
estimated for every meter of structure installed.
construction site into the building.
The steel structures that arrive on site are positioned manually Name Value Unit
and installed using a drill to screw the screws to hold the Electricity consumption 0.0208 kWh
various structural parts (studs, tracks etc.) together, ready to
contain the plasterboard wall or ceiling that will be placed there,
without the need for auxiliary materials.
4 Environmental Product Declaration - Etex Building Performance SpA - PregyMetal AquaBoard - AZ150 galvanized steel profiles with 0,6mm thickness
In case a reference service life according to applicable ISO
End of life (C1 - C4)
standards is declared then the assumptions and in-use
C1:The product dismantling from the building is done manually
conditions underlying the determined RSL shall be declared. In
through the use of a drill to unscrew the screws that hold the
addition, it shall be stated that the RSL applies to the reference
channels, studs and tracks together.
conditions only.
C2: 100 km estimated
C3: 90% of product mass is recycled
The same holds for a service life declared by the manufacturer.
C4: 10% of product mass is send to landfill
Corresponding information related to in-use conditions needs
not be provided if a service life taken from the list of service life Name Value Unit
by BNB is declared. Recycling 0.9 kg
Landfilling 0.1 kg
Reference service life
Name ValueUnit
Life Span (according to BBSR) 50 a
Maintenance e.g. required frequency, type and
- -
quality and replacement of components
5 Environmental Product Declaration - Etex Building Performance SpA - PregyMetal AquaBoard - AZ150 galvanized steel profiles with 0,6mm thickness
5. LCA: Results
The following table shows the result of the LCA for 1 kg of the reference product. The results in the B module are based on a period of
one year as no reference service life is declared. The environmental impact due to the use phase is null.
DESCRIPTION OF THE SYSTEM BOUNDARY (X = INCLUDED IN LCA; MND = MODULE OR INDICATOR NOT DECLARED; MNR
= MODULE NOT RELEVANT)
Benefits and
Construction loads beyond
Product stage Use stage End of life stage
process stage the system
boundaries
la ire ta m w a Ry lp p u s tro p s n a rT g n iru tc a fu n a M e h t m o rf tro p s n a rTe tis e h t o t e ta g y lb m e s s A e s U e c n a n e tn ia M ria p e R tn e m e c a lp e R tn e m h s ib ru fe R y g re n e la n o ita re p Oe s u re ta w la n o ita re p Oe s u n o itc u rts n o c -e Dn o itilo m e d tro p s n a rT g n is s e c o rp e ts a W la s o p s iD -e s u e R-y re v o c e R-g n ilc y c e Rla itn e to p
A1 A2 A3 A4 A5 B1 B2 B3 B4 B5 B6 B7 C1 C2 C3 C4 D
X X X MND X MND MND MNR MNR MNR MND MND X X X X X
RESULTS OF THE LCA - ENVIRONMENTAL IMPACT according to EN 15804+A2: 1 Kg Average PregyMetal AquaBoard - AZ150
galvanized steel profiles with 0,6mm thickness
Parameter Unit A1 A2 A3 A5 C1 C2 C3 C4 D
GWP-total kg CO 2 eq 2.47E+00 9.5E-02 2.84E-03 1.33E-02 1.29E-02 1.92E-02 1.73E-02 6.35E-04 -1.2E+00
GWP-fossil kg CO 2 eq 2.46E+00 9.49E-02 3.33E-03 1.23E-02 1.18E-02 1.92E-02 1.73E-02 6.34E-04 -1.19E+00
GWP-biogenic kg CO 2 eq 2.16E-03 9.11E-05 -4.86E-04 1.57E-03 1.08E-03 1.84E-05 1.66E-05 4.1E-07 -2.43E-03
GWP-luluc kg CO 2 eq 2.05E-03 4.56E-05 2.68E-06 2.02E-06 1.81E-06 9.21E-06 8.29E-06 3.73E-07 -5.12E-04
ODP kg CFC11 eq 6.1E-08 2.02E-09 1.59E-10 2.67E-10 2.57E-10 4.09E-10 3.68E-10 1.76E-11 -2.19E-08
AP mol H+ eq 4.32E-02 3.83E-04 1.38E-05 4.32E-05 4.14E-05 7.74E-05 6.97E-05 4.58E-06 -4.86E-03
EP-freshwater kg P eq 1.14E-03 6.52E-06 7.06E-07 1.85E-06 1.82E-06 1.32E-06 1.19E-06 5.06E-08 -5.55E-04
EP-marine kg N eq 3.36E-03 1.46E-04 2.78E-06 7.74E-06 7.08E-06 2.95E-05 2.66E-05 1.76E-06 -1.08E-03
EP-terrestrial mol N eq 1.64E-01 1.56E-03 2.7E-05 8.74E-05 8.04E-05 3.15E-04 2.84E-04 1.88E-05 -1.15E-02
kg NMVOC
POCP 1.15E-02 5.61E-04 5.23E-05 3.7E-05 3.45E-05 1.13E-04 1.02E-04 6.56E-06 -5.46E-03
eq
ADPE kg Sb eq 2.75E+01 1.32E+00 1.1E-01 1.87E-01 1.8E-01 2.67E-01 2.4E-01 1.51E-02 -1.19E+01
ADPF MJ 4.78E-05 2.99E-07 2.3E-08 2.18E-08 2.04E-08 6.04E-08 5.44E-08 8.44E-10 -9.83E-06
m3 world eq
WDP 8.27E-01 5.45E-03 6.73E-04 7.26E-03 7.24E-03 1.1E-03 9.92E-04 6.7E-04 -2.45E-01
deprived
GWP = Global warming potential; ODP = Depletion potential of the stratospheric ozone layer; AP = Acidification potential of land and water; EP =
Eutrophication potential; POCP = Formation potential of tropospheric ozone photochemical oxidants; ADPE = Abiotic depletion potential for non-fossil
resources; ADPF = Abiotic depletion potential for fossil resources; WDP = Water (user) deprivation potential)
RESULTS OF THE LCA - INDICATORS TO DESCRIBE RESOURCE USE according to EN 15804+A2: 1 Kg Average PregyMetal
AquaBoard - AZ150 galvanized steel profiles with 0,6mm thickness
Parameter Unit A1 A2 A3 A5 C1 C2 C3 C4 D
PERE MJ 2.24E+00 2.05E-02 1.26E-02 4.58E-02 4.56E-02 4.14E-03 3.73E-03 1.28E-04 0
PERM MJ 0 0 0 0 0 0 0 0 0
PERT MJ 2.24E+00 2.05E-02 1.26E-02 4.58E-02 4.56E-02 4.14E-03 3.73E-03 1.28E-04 0
PENRE MJ 2.92E+01 1.4E+00 1.17E-01 2.02E-01 1.95E-01 2.84E-01 2.55E-01 1.61E-02 0
PENRM MJ 0 0 0 0 0 0 0 0 0
PENRT MJ 2.92E+01 1.4E+00 1.17E-01 2.02E-01 1.95E-01 2.84E-01 2.55E-01 1.61E-02 0
SM kg 3.5E-01 0 0 0 0 0 0 0 0
RSF MJ 0 0 0 0 0 0 0 0 0
NRSF MJ 0 0 0 0 0 0 0 0 0
FW m3 2.48E-02 1.88E-04 2.24E-05 1.95E-04 1.94E-04 3.8E-05 3.42E-05 1.61E-05 -6.69E-03
PERE = Use of renewable primary energy excluding renewable primary energy resources used as raw materials; PERM = Use of renewable primary
energy resources used as raw materials; PERT = Total use of renewable primary energy resources; PENRE = Use of non-renewable primary energy
excluding non-renewable primary energy resources used as raw materials; PENRM = Use of non-renewable primary energy resources used as raw
materials; PENRT = Total use of non-renewable primary energy resources; SM = Use of secondary material; RSF = Use of renewable secondary fuels;
NRSF = Use of non-renewable secondary fuels; FW = Use of net fresh water
RESULTS OF THE LCA – WASTE CATEGORIES AND OUTPUT FLOWS according to EN 15804+A2:
1 Kg Average PregyMetal AquaBoard - AZ150 galvanized steel profiles with 0,6mm thickness
Parameter Unit A1 A2 A3 A5 C1 C2 C3 C4 D
HWD kg 4.34E-04 8.4E-06 5.72E-07 6.47E-07 6.07E-07 1.7E-06 1.53E-06 8.02E-08 -1.01E-04
NHWD kg 5.9E-01 6.45E-02 3.69E-04 7.96E-04 5.37E-04 1.3E-02 1.17E-02 1E-01 -4.95E-01
RWD kg 4.28E-05 4.29E-07 6.98E-08 3.92E-07 3.9E-07 8.67E-08 7.8E-08 2.24E-09 -1.05E-05
CRU kg 0 0 0 0 0 0 0 0 0
MFR kg 0 0 9.5E-03 2E-02 0 0 9E-01 0 0
6 Environmental Product Declaration - Etex Building Performance SpA - PregyMetal AquaBoard - AZ150 galvanized steel profiles with 0,6mm thickness
MER kg 0 0 0 0 0 0 0 0 0
EEE MJ 0 0 0 0 0 0 0 0 0
EET MJ 0 0 0 0 0 0 0 0 0
HWD = Hazardous waste disposed; NHWD = Non-hazardous waste disposed; RWD = Radioactive waste disposed; CRU = Components for re-use;
MFR = Materials for recycling; MER = Materials for energy recovery; EEE = Exported electrical energy; EET = Exported thermal energy
RESULTS OF THE LCA – additional impact categories according to EN 15804+A2-optional:
1 Kg Average PregyMetal AquaBoard - AZ150 galvanized steel profiles with 0,6mm thickness
Parameter Unit A1 A2 A3 A5 C1 C2 C3 C4 D
Disease
PM 4.82E-07 7.58E-09 1.53E-10 2.28E-10 1.97E-10 1.53E-09 1.38E-09 1E-10 -8.72E-08
incidence
IR kBq U235 eq 1.69E-01 1.77E-03 2.78E-04 1.5E-03 1.49E-03 3.57E-04 3.21E-04 9.59E-06 -4.16E-02
ETP-fw CTUe 2.4E+01 6.97E-01 4.32E-02 2.53E-02 2.2E-02 1.41E-01 1.27E-01 7.43E-03 -2.96E+00
HTP-c CTUh 6.92E-08 1.22E-09 5.46E-11 7.83E-11 7.28E-11 2.47E-10 2.22E-10 7.34E-12 -2.86E-08
HTP-nc CTUh 1.54E-08 4.23E-11 2.72E-12 3.24E-12 3.06E-12 8.54E-12 7.69E-12 2.59E-13 -7.25E-09
SQP SQP 8.5E+00 7.85E-01 6.38E-02 3.09E-02 2.77E-02 1.59E-01 1.43E-01 3.01E-02 -3.81E+00
PM = Potential incidence of disease due to PM emissions; IR = Potential Human exposure efficiency relative to U235; ETP-fw = Potential comparative
Toxic Unit for ecosystems; HTP-c = Potential comparative Toxic Unit for humans (cancerogenic); HTP-nc = Potential comparative Toxic Unit for humans
(not cancerogenic); SQP = Potential soil quality index
Disclaimer 1 – for the indicator “Potential Human exposure efficiency relative to U235”. This impact category deals mainly with the
eventual impact of low-dose ionizing radiation on human health of the nuclear fuel cycle. It does not consider effects due to possible
nuclear accidents, occupational exposure or radioactive waste disposal in underground facilities. Potential ionizing radiation from the
soil, radon and from some construction materials is also not measured by this indicator.
Disclaimer 2 – for the indicators “abiotic depletion potential for non-fossil resources”, “abiotic depletion potential for fossil resources”,
“water (user) deprivation potential, deprivation-weighted water consumption”, “potential comparative toxic unit for ecosystems”,
“potential comparative toxic unit for humans – cancerogenic”, “Potential comparative toxic unit for humans - not cancerogenic”,
“potential soil quality index”. The results of this environmental impact indicator shall be used with care as the uncertainties on these
results are high as there is limited experience with the indicator.
6. LCA: Interpretation
Product stage (modules A1-A3) is responsible for the biggest impacts on the Global Warming Potential is due to its
share of the impact for most indicators. About 90% of the production, especially in the raw materials phase in A1.
7. Requisite evidence
The products covered by this document comply with EN 14195 type of surface treatment.
regarding their field of application and with EN 10346 for the
8. References
Standards Institut Bauen und Umwelt e.V.: General Instructions for the
EPD programme of Institut Bauen und Umwelt e.V., Version
EN 15804 2.0, Berlin: Institut Bauen und Umwelt e.V., 2021
www.ibu-epd.com
EN 15804:2012+A1 2013, Sustainability of construction works
— Environmental Product Declarations — Core rules for the Standards:
product category of construction products.
EN 15804 EN 15804EN 15804:2012+A1 2013, Sustainability of
construction works— Environmental Product Declarations —
EN 15804:2012+A2:2019+AC:2021, Sustainability of Core rules for theproduct category of construction products.EN
construction works — Environmental Product Declarations — 15804.
Core rules for the product category of construction products.
EN 15804:2012+A2:2019+AC:2021, Sustainability
ISO 14025 ofconstruction works — Environmental Product Declarations —
Core rules for the product category of construction
EN ISO 14025:2011, Environmental labels and declarations — products.ISO 14025.
Type III environmental declarations — Principles and
procedures. EN ISO 14025:2011, Environmental labels and declarations —
Type III environmental declarations — Principles
Further References andprocedures.
Title of the software/database EN 14195:2005 - Metal framing components for gypsum board
systems - Definitions, requirements and test methods and the
Title of the software/database. Addition to the title, version.
CE-marking.
Place: Publisher, Date of publication [Access on access date].
UNI EN ISO 9001:2015 - Quality management systems
IBU 2021
7 Environmental Product Declaration - Etex Building Performance SpA - PregyMetal AquaBoard - AZ150 galvanized steel profiles with 0,6mm thickness
UNI ISO 45001:2018 - Occupational health and safety
management systems PCR Part A - Calculation Rules for the Life Cycle As-sessment
and Requirements on the Project Re-port according to EN
UNI EN ISO 14001:2015 - Environmental management 15804+A2:2019. Version 6, 12/07/2023
systems
PCR Part B - Requiment on the EPD for Structural steel, V.1,
ISO 15686 - Buildings and constructed assets 06/04/2023.
ISO 13501:1 - Petroleum and natural gas industries Regulation (EU) No. 305/2011 -Regulation (EU) No 305/2011 of
the European Parliament and of the Council of 9 March 2011
European Regulation EC/1272/2008 -Regulation (EC) No laying down harmonised conditions for the marketing of
1272/2008 of the European Parliament and of the Council of 16 construction products and repealing Council Directive
December 2008 on classification, labelling and packaging of 89/106/EEC Text with EEA relevance
substances and mixtures, amending and repealing Directives
67/548/EEC and 1999/45/EC, and amending Regulation (EC) Candidate List of Substances of Very High Concern for
No 1907/2006 (Text with EEA relevance) Authorisation' (SVHC).
EN 14195 - Metal framing components for gypsum board EWC-Stat categories - European Waste Classification.
systems
Federal office for building and regional planning (BBSR) BNB
EN 10346 - Continuously hot-dip coated steel flat products " (http://www.nachhaltigesbauen.de/baustoff-und-
gebaeudedaten/nutzungsdauern-von-bauteilen.html).
Further References:
Title of the software/database:
IBU 2021
Institut Bauen und Umwelt e.V.: General Instructions for Software: SimaPro 9.5.0.1
theEPD programme of Institut Bauen und Umwelt e.V., Database: Ecoinvent 3.9.1
Version2.0, Berlin: Institut Bauen und Umwelt e.V.,
2021www.ibu-epd.com.
8 Environmental Product Declaration - Etex Building Performance SpA - PregyMetal AquaBoard - AZ150 galvanized steel profiles with 0,6mm thickness
Publisher
Institut Bauen und Umwelt e.V. +49 (0)30 3087748- 0
Hegelplatz 1 info@ibu-epd.com
10117 Berlin www.ibu-epd.com
Germany
Programme holder
Institut Bauen und Umwelt e.V. +49 (0)30 3087748- 0
Hegelplatz 1 info@ibu-epd.com
10117 Berlin www.ibu-epd.com
Germany
Author of the Life Cycle Assessment
Greenwich srl +390354948794
Via Presolana 2/4 info@greenwichsrl.it
24030 Medolago https://greenwichsrl.it/
Italy
Owner of the Declaration
Etex Building Performance International +32 2 778 12 11
Rue Marcel Demonque 500 info@etexgroup.com
84915 Avignon Cedex 9 www.etexgroup.com
France
9 Environmental Product Declaration - Etex Building Performance SpA - PregyMetal AquaBoard - AZ150 galvanized steel profiles with 0,6mm thickness
