ENVIRONMENTAL PRODUCT DECLARATION
as per ISO 14025 and EN 15804+A2
Owner of the Declaration Ideal standard International
Publisher Institut Bauen und Umwelt e.V. (IBU)
Programme holder Institut Bauen und Umwelt e.V. (IBU)
Declaration number EPD-IDE-20230006-IBD1-EN
Issue date 24.05.2023
Valid to 23.05.2028
Ceramic Fine Fireclay ISI
Ideal Standard International
www.ibu-epd.com | https://epd-online.com
1. General Information
Ideal Standard International Ceramic Fine Fireclay ISI
Programme holder Owner of the declaration
IBU – Institut Bauen und Umwelt e.V. Ideal standard International
Hegelplatz 1 Da Vincilaan 2
10117 Berlin 1935 Zaventem Belgium
Germany France
Declaration number Declared product / declared unit
EPD-IDE-20230006-IBD1-EN 1 kg of ceramic fine fireclay product
This declaration is based on the product category rules: Scope:
Sanitary ceramics, 01.08.2021 The EPD contains the result of 1 kg of ceramic Fine fire clay product
(PCR checked and approved by the SVR) produced by Ideal Standard. It is representative for the following ceramic
products categories: bathroom basin ceramic, bidet, pedestal/semi-
pedestal and washstand basin ceramic) manufactured in Armitage (United
Issue date Kingdom) and Teplice (Czech Republique). As the result is for 1kg of
ceramic, the user can easily calculate the results for ceramic products,
24.05.2023
noted above according to the weight.
Foreground data has been provided directly by Ideal Standard and
Valid to
background LCA data is based on Ecoinvent 3.8 and Industry 2.0 data.
23.05.2028 The owner of the declaration shall be liable for the underlying information
and evidence; the IBU shall not be liable with respect to manufacturer
information, life cycle assessment data and evidences.
The EPD was created according to the specifications of EN 15804+A2. In
the following, the standard will be simplified as EN 15804.
Verification
The standard EN 15804 serves as the core PCR
Independent verification of the declaration and data according to ISO
14025:2011
Dipl.-Ing. Hans Peters internally X externally
(Chairman of Institut Bauen und Umwelt e.V.)
Florian Pronold Vito D'Incognito,
(Managing Director Institut Bauen und Umwelt e.V.) (Independent verifier)
1 Environmental Product Declaration - Ideal Standard International - Ceramic Fine Fireclay ISI
2. Product
substances listed in the candidate list (date: 16.05.2023)
2.1 Product description/Product definition exceeding 0.1 percentage by mass: no
This declaration covers 1 kg of standard white Fine Fire Clay
product. Product categories included in this EPD are: bowls This product/article/at least one partial article contains other
(bathroom basin ceramic, bidet, pedestal/semi-pedestal and carcinogenic, mutagenic, reprotoxic (CMR) substances in
washstand basin ceramic, manufactured in Teplice (Czech categories 1A or 1B which are not on the candidate list,
Republique) and Armitage (UK). exceeding 0.1 percentage by mass: no
The EPD is based on average data between both plants. A Biocide products were added to this construction product or it
variability study is performed to show the representativeness of has been treated with biocide products (this then concerns a
the average for both plants. treated product as defined by the (EU) Ordinance on Biocide
Products No. 528/2012): no
The manufacturer can - within the framework of the European
Regulation N° 305/2011 (CPR) - present the Declaration of 2.6 Manufacture
Performance (DOP) of the product confirming that the product
1. Slip preparation Production of the ceramic mixture (slip)
has a CE marking.
and unloading/storage of raw materials in the area.
2. Glaze preparation Production of glaze with needed
2.2 Application
colour.
The products/solutions are used in private and public
3. Casting shop Casting of ceramic products in different
bathrooms. The product can be used in new construction and
moulds.
renovation work for hygienic and household use.
4. Dryers Drying is the process of taking off the humidity
2.3 Technical Data and the final results are dried products.
5. White inspection The first inspection of dried ceramic
Constructional data products. The main focus is checking the quality and
Name Value Unit cleaning the surface of the products. At the end of the
Crazing test 1hr in autoclave with 5 bar process the products are grouped in three different
-
steam directions: A grade products, products for repair and
scrap.
Minimum 1
Impact resistance Ball bearing dropped 6. Spraying Covering the ceramic product with glaze
drop without N/cm
from fixed height 7. Kilns Firing of ceramic products
breaking
8. Gloss inspection Final inspection for visual control of all
Resistance to chemicals and staining
products for visible defects. Separating the products
EN14688 for Wash Basins therefore by
No remaining again into three groups: for packaging, for repairing by
extension to other Ceramic Products.
chemical - hand or for grinding machines and scrap (pitcher).
Specific chemicals in contact then
evident 9. Packaging Different kinds of activities for the packaging
cleaned with specific apparatus without
of the products.
permanent marking
*Moulds making Development of a new matrix for the
Resistance to temperature change production of gypsum moulds for casting and repairing the
EN14688 for Wash basins. 1000 hot (75 No visible - damaged matrix.
degC) / cold (15 degC) water cycles damage
withut visible damage *Mould shop Production of gypsum moulds for casting ceramic
Load resistance 150 kg products and polyurethane setters for supporting the casting
Resistance to abrasion EN14688 for process.
Wash Basins therefore by extension to No scratches
2.7 Environment and health during manufacturing
other Ceramic Products. Loaded diamond through outer
tool (scratch) / Loaded abrasive paper (glaze) layer Environmental, occupational health, safety and quality
wheel (abrasion) for repeated cycles. management at the Ideal Standard plants are in accordance
with the following standards:
The manufacturer can - within the framework of the European
• ISO 14001
Regulation N° 305/2011 (CPR) - present the Declaration of
• ISO 9001
Performance (DOP) of the product confirming that the product
• ISO 45001
has a CE marking.
2.8 Product processing/Installation
2.4 Delivery status
It is considered that there is no assembly waste, based on the
The products are packed: wooden pallet, PE plastic and
fact that the product is prefabricated and installed by hand.
cardboard, and are accompanied with an instruction and
guarantee sheet. The products can come in different shapes
2.9 Packaging
and dimensions. An overview of all included products in this
A wooden pallet, PE plastic bag and cardboard are used to
EPD can be provided by Ideal Standard.
pack and transport the product to the supplier/customer. The
2.5 Base materials/Ancillary materials product is also accompanied by an instruction and guarantee
sheet.
This EPD includes different product categories: bathroom
basin, bidet, pedestal/semi-pedestal, and washstand basin: the
2.10 Condition of use
Fine Fire Clay ceramic is composed of Chamotte - ground fired
The product will not change in material composition over its
clay, Clay - Ball clay, Sand as silica and Glaze.
use.
This product/article/at least one partial article contains 2.11 Environment and health during use
2 Environmental Product Declaration - Ideal Standard International - Ceramic Fine Fireclay ISI
Under normal conditions of use, the product does not cause occur in terms of environment and human health.
any adverse health effects or release of volatile organic
compounds (VOCs) into indoor air. 2.14 Re-use phase
It is possible to recycle ceramic products in the production
No environmental impact on water, air or soil is expected. process. This is already applied to production waste. The
recycling of post-consumer waste depends on the sorting and
2.12 Reference service life take-back of these waste streams at the demolition site.
The reference service life is not relevant, as module B is not
considered. 2.15 Disposal
According to the average European end-of-life scenario
2.13 Extraordinary effects described in Annexe C of the Product Environmental Footprint
Fire Pilots (PEFCR) 6.3 guidance, the following disposal scenarios
Not subjected to fire classification have been considered: 100 % of the ceramic is landfilled.
Water
No risks are expected to occur in terms of environmental and 2.16 Further information
human health. Additional information on Fine Fire Clay ceramic products
manufactured by Ideal Standard can be found on:
Mechanical destruction https://www.idealstandard.com/
In case of mechanical destruction, no risks are expected to
3. LCA: Calculation rules
materials and smaller waste flows have been excluded).
3.1 Declared Unit • Only the most relevant ancillary materials have been
The EPD is relevant to1kg of Fine Fire Clay ceramic product. selected based on consumption rate and importance in
the production process.
The EPD is based on average data of the different plants, • Environmental impacts caused by the personnel of the
Teplice (CZ) and Armitage (UK). A variability study is performed production plants are not included in the LCA, e.g.
to show the representativeness of the average for both plants. waste from the cafeteria and sanitary installations or
environmental effects caused by commuter traffic.
The variability between the Armitage plant against the average Cooling of the plants in order to ensure a comfortable
is less than 30%. indoor climate for the personnel for example is also
neglected.
The variability between the Teplice plant against the average is
less than 30%. 3.5 Background data
Ecoinvent 3.8 and Industry 2.0
Declared unit
Name Value Unit 3.6 Data quality
Declared unit 0.001 t Foreground data is specific to Ideal Standard and is collected
for the reference year 2021. Background data is based on
As the result is for 1kg of ceramic, the user can easily calculate
Ecoinvent 3.8 which is released in September 2021.
the results for ceramic products, as noted above according to
the weight. The products typically weigh between 4 and 32 kg.
This LCA study is looking at 1 kg of ceramic Fine fire clay
products. This ceramic is manufactured in Armitage (United
3.2 System boundary Kingdom) or Teplice (Czech Republique). The variability
Cradle-to-gate with options, including modules A4, A5, C1, C2, between the Armitage plant against the average (between the
C3, C4 and D Armitage and Teplice plant) is less than 30%.
3.3 Estimates and assumptions The variability between the Teplice plant against the average
The following processes are excluded because data was not (between the Armitage and Teplice plant) is less than 30%.
available:
3.7 Period under review
• Packaging of the raw materials used to produce the
The data collected by Ideal Standard is based on data from the
glaze of the ceramic products
production year 2021.
• Transport of Ball clay raw material to CZ plant
• Transport packaging final product 3.8 Geographic Representativeness
• Ancillary materials in CZ plant Land or region, in which the declared product system is
• Packaging and transport of ancillary materials used manufactured, used or handled at the end of the product´s
during the production process lifespan: Europe
• Packaging and transport of ancillary materials used
during installation
No further approximations have been made to replace the 3.9 Allocation
missing data, as they were considered to be not relevant based Amounts of the raw materials/components (modules A1 and A2)
on the first iterations of the results. and the packaging of the final product have been extracted
from recipes used in the respective factory. No allocation was
3.4 Cut-off criteria
necessary. Note that the production losses have been added to
The following processes are considered below cut-off: the recipe.
• Big bags used as packaging of some raw materials for
the ceramic production, as they are reused. The data for the production process (module A3) i.e. input and
• For production waste only the most relevant production outputs such as energy consumption, water consumption,
waste streams have been considered (waste of ancillary production waste, ancillary materials and emissions are based
3 Environmental Product Declaration - Ideal Standard International - Ceramic Fine Fireclay ISI
on factory averages (total amount in the factory converted to 1 according to EN 15804 and the building context, respectively
kg based on the total production volume in kg). the product-specific characteristics of performance, are taken
into account. The used background database are Ecoinvent 3.8
3.10 Comparability and Industry 2.0.
Basically, a comparison or an evaluation of EPD data is only
possible if all the data sets to be compared were created
4. LCA: Scenarios and additional technical information
End of life (C1-C4)
Characteristic product properties of biogenic carbon
According to the average European end-of-life scenario
The product does not contain biogenic carbon, but its
described in Annexe C of the Product Environmental Footprint
accompanying packaging contains 8.77E-02 kg C per product
Pilots (PEFCR) 6.3 guidance, the following disposal scenarios
in the form of paper, cardboard and wooden pallets.
have been considered: 100% of the ceramic parts are
Information on describing the biogenic Carbon Content at landfilled.
factory gate
Name Value Unit
Name Value Unit
Collected separately waste type waste type 1 kg
kg
Biogenic carbon content in product - Landfilling 1 kg
C
Biogenic carbon content in accompanying kg Reuse, recovery and/or recycling potentials (D), relevant
0.0877
packaging C scenario information
Module D contains low benefits and loads of recycling of the
packaging of the final product and the benefits of energy
recovery during the incineration of the plastic. There are no
Transport to the building site (A4)
benefits and loads from the end of life of the product, because
Name Value Unit the product is 100 % landfilled.
Litres of fuel 260 l/100km Name Value Unit
Transport distance 2000 km
Capacity utilisation (including empty runs) - %
Gross density of products transported - kg/m3
Capacity utilisation volume factor - -
Installation into the building (A5)
It is considered that there is no assembly waste, based on the
fact that the product is prefabricated and installed by hand.
Only the impact of packaging waste has been considered.
Name Value Unit
Packaging waste (paper and cardboard) PEF
EOL scenario Europe for coverage carton
0,085 Kg
packaging: 11 % incineration; 75 % recycling;
14 % landfill
Packaging waste (PE) PEF EOL scenario
Europe for PE packaging: 32 % incineration; 29 0,039338 Kg
% recycling; 39 % landfill
Packaging waste (wooden pallet) PEF EOL
scenario Europe for wooden pallets: 32 % 0,110 Kg
incineration; 30 % recycling; 38 % landfill
4 Environmental Product Declaration - Ideal Standard International - Ceramic Fine Fireclay ISI
5. LCA: Results
DESCRIPTION OF THE SYSTEM BOUNDARY (X = INCLUDED IN LCA; ND = MODULE OR INDICATOR NOT DECLARED; MNR =
MODULE NOT RELEVANT)
Benefits and
Construction loads beyond
Product stage Use stage End of life stage
process stage the system
boundaries
la ire ta m w a Ry lp p u s tro p s n a rT g n iru tc a fu n a M e h t m o rf tro p s n a rTe tis e h t o t e ta g y lb m e s s A e s U e c n a n e tn ia M ria p e R tn e m e c a lp e R tn e m h s ib ru fe R y g re n e la n o ita re p Oe s u re ta w la n o ita re p Oe s u n o itc u rts n o c -e Dn o itilo m e d tro p s n a rT g n is s e c o rp e ts a W la s o p s iD -e s u e R-y re v o c e R-g n ilc y c e Rla itn e to p
A1 A2 A3 A4 A5 B1 B2 B3 B4 B5 B6 B7 C1 C2 C3 C4 D
X X X X X MND MND MNR MNR MNR MND MND X X X X X
RESULTS OF THE LCA - ENVIRONMENTAL IMPACT according to EN 15804+A2: 1 Kg Declared unit
Parameter Unit A1 A2 A3 A4 A5 C1 C2 C3 C4 D
GWP-total kg CO 2 eq 2.82E-01 3.53E-02 1.43E+00 3.93E-01 3.1E-01 1.54E-04 8.15E-03 0 6.08E-03 -1.67E-01
GWP-fossil kg CO 2 eq 2.81E-01 3.53E-02 1.7E+00 3.93E-01 3.04E-02 1.52E-04 8.14E-03 0 6.06E-03 -4.7E-02
GWP-
biogenic kg CO 2 eq 7.44E-04 1.16E-05 -2.71E-01 1.4E-04 2.79E-01 8.44E-07 2.91E-06 0 1.15E-05 -1.19E-01
GWP-luluc kg CO 2 eq 9.57E-05 1.62E-05 1.01E-03 1.57E-04 2.77E-06 3.6E-07 3.26E-06 0 4.47E-06 -1.3E-04
ODP kg CFC11 eq 3.96E-08 7.93E-09 2.07E-07 9.1E-08 1.43E-09 7.66E-12 1.89E-09 0 2.25E-09 -4.67E-09
AP mol H+ eq 1.01E-03 3.4E-04 3.8E-03 1.12E-03 3.85E-05 8.65E-07 2.31E-05 0 5.35E-05 -2.07E-04
EP-
kg P eq 7.51E-06 2.23E-07 5.03E-05 2.8E-06 7.31E-08 1.63E-08 5.81E-08 0 1.86E-07 -2.46E-06
freshwater
EP-marine kg N eq 3.51E-04 8.96E-05 8.21E-04 2.22E-04 1.51E-05 1.1E-07 4.6E-06 0 1.83E-05 -5.07E-05
EP-terrestrial mol N eq 3.92E-03 9.93E-04 9.17E-03 2.47E-03 1.52E-04 1.27E-06 5.12E-05 0 2.02E-04 -5.57E-04
kg NMVOC
POCP 1.11E-03 2.75E-04 2.59E-03 9.49E-04 4.55E-05 3.5E-07 1.97E-05 0 5.74E-05 -1.9E-04
eq
ADPE kg Sb eq 7.75E-07 8.26E-08 2.24E-06 1.06E-06 1.7E-08 8.23E-10 2.21E-08 0 1.44E-08 -1.54E-07
ADPF MJ 4.22E+00 5.17E-01 3.24E+01 5.95E+00 9.74E-02 3.23E-03 1.23E-01 0 1.73E-01 -1.05E+00
m3 world eq
WDP 3.97E-02 1.44E-03 4.48E-01 1.81E-02 5.66E-04 3.78E-05 3.76E-04 0 8.11E-04 -4.52E-02
deprived
GWP = Global warming potential; ODP = Depletion potential of the stratospheric ozone layer; AP = Acidification potential of land and water; EP =
Eutrophication potential; POCP = Formation potential of tropospheric ozone photochemical oxidants; ADPE = Abiotic depletion potential for non-fossil
resources; ADPF = Abiotic depletion potential for fossil resources; WDP = Water (user) deprivation potential)
RESULTS OF THE LCA - INDICATORS TO DESCRIBE RESOURCE USE according to EN 15804+A2: 1 Kg Declared unit
Parameter Unit A1 A2 A3 A4 A5 C1 C2 C3 C4 D
PERE MJ 1.47E-01 6.52E-03 2.51E+00 8.37E-02 6.83E-01 6.41E-04 1.74E-03 0 8.94E-03 0
PERM MJ 0 0 2.37E+00 0 -1.55E+00 0 0 0 0 8.68E-01
PERT MJ 1.47E-01 6.52E-03 4.88E+00 8.37E-02 -8.65E-01 6.41E-04 1.74E-03 0 8.94E-03 8.68E-01
PENRE MJ 4.75E+00 5.19E-01 3.59E+01 5.99E+00 2.15E-01 3.83E-03 1.24E-01 0 1.78E-01 0
PENRM MJ 0 0 3.59E-01 0 -2.19E-01 0 0 0 0 1.04E-01
PENRT MJ 4.75E+00 5.19E-01 3.62E+01 5.99E+00 -4.32E-03 3.83E-03 1.24E-01 0 1.78E-01 1.04E-01
SM kg 0 0 0 0 0 0 0 0 0 6.23E-02
RSF MJ 0 0 0 0 0 0 0 0 0 0
NRSF MJ 0 0 0 0 0 0 0 0 0 0
FW m3 3.67E-04 3.38E-05 1.33E-02 4.38E-04 5.26E-05 2.43E-06 9.08E-06 0 1.86E-04 -1.08E-03
PERE = Use of renewable primary energy excluding renewable primary energy resources used as raw materials; PERM = Use of renewable primary
energy resources used as raw materials; PERT = Total use of renewable primary energy resources; PENRE = Use of non-renewable primary energy
excluding non-renewable primary energy resources used as raw materials; PENRM = Use of non-renewable primary energy resources used as raw
materials; PENRT = Total use of non-renewable primary energy resources; SM = Use of secondary material; RSF = Use of renewable secondary fuels;
NRSF = Use of non-renewable secondary fuels; FW = Use of net fresh water
RESULTS OF THE LCA – WASTE CATEGORIES AND OUTPUT FLOWS according to EN 15804+A2:
1 Kg Declared unit
Parameter Unit A1 A2 A3 A4 A5 C1 C2 C3 C4 D
HWD kg 6.68E-06 1.2E-06 4.64E-05 1.55E-05 2.32E-07 2.45E-09 3.22E-07 0 1.9E-07 -8.96E-07
NHWD kg 1.45E-02 2.23E-02 1.26E-01 3.12E-01 7.03E-02 1.18E-05 6.47E-03 0 1E+00 -5.89E-03
RWD kg 1.04E-05 3.51E-06 9.76E-05 4.02E-05 6.31E-07 2.36E-08 8.34E-07 0 1.18E-06 -2.86E-06
CRU kg 0 0 0 0 0 0 0 0 0 0
MFR kg 0 0 0 0 6.23E-02 0 0 0 0 -6.23E-02
MER kg 0 0 0 0 0 0 0 0 0 0
EEE MJ 0 0 0 0 1.59E-01 0 0 0 0 -1.59E-01
EET MJ 0 0 0 0 7.95E-02 0 0 0 0 -7.95E-02
5 Environmental Product Declaration - Ideal Standard International - Ceramic Fine Fireclay ISI
HWD = Hazardous waste disposed; NHWD = Non-hazardous waste disposed; RWD = Radioactive waste disposed; CRU = Components for re-use;
MFR = Materials for recycling; MER = Materials for energy recovery; EEE = Exported electrical energy; EET = Exported thermal energy
RESULTS OF THE LCA – additional impact categories according to EN 15804+A2-optional:
1 Kg Declared unit
Parameter Unit A1 A2 A3 A4 A5 C1 C2 C3 C4 D
Disease
PM 1.85E-08 2.65E-09 2.98E-08 3.15E-08 6.7E-10 2.39E-12 6.54E-10 0 1.04E-09 -4.11E-09
incidence
IR kBq U235 eq 7.31E-03 2.24E-03 1.31E-01 2.58E-02 4.32E-04 2.86E-05 5.36E-04 0 8.85E-04 -3.02E-03
ETP-fw CTUe 1.93E+00 3.89E-01 8.06E+00 4.67E+00 1E-01 2.04E-03 9.69E-02 0 9.95E-02 -4.89E-01
HTP-c CTUh 1.01E-10 1.5E-11 6.28E-10 1.5E-10 1.93E-11 6.27E-14 3.12E-12 0 2.89E-12 -1.99E-11
HTP-nc CTUh 1.88E-09 3.86E-10 6.59E-09 4.72E-09 1.41E-10 2E-12 9.79E-11 0 5.84E-11 -4.51E-10
SQP SQP 1.45E+00 3.06E-01 2.54E+01 4.15E+00 9.1E-02 5.85E-04 8.6E-02 0 3.27E-01 -1.28E+01
PM = Potential incidence of disease due to PM emissions; IR = Potential Human exposure efficiency relative to U235; ETP-fw = Potential comparative
Toxic Unit for ecosystems; HTP-c = Potential comparative Toxic Unit for humans (cancerogenic); HTP-nc = Potential comparative Toxic Unit for humans
(not cancerogenic); SQP = Potential soil quality index
Disclaimer 1 – for the indicator “Potential Human exposure efficiency relative to U235”. This impact category deals mainly with the
eventual impact of low-dose ionizing radiation on human health of the nuclear fuel cycle. It does not consider effects due to possible
nuclear accidents, occupational exposure or radioactive waste disposal in underground facilities. Potential ionizing radiation from the
soil, radon and from some construction materials is also not measured by this indicator.
Disclaimer 2 – for the indicators “abiotic depletion potential for non-fossil resources”, “abiotic depletion potential for fossil resources”,
“water (user) deprivation potential, deprivation-weighted water consumption”, “potential comparative toxic unit for ecosystems”,
“potential comparative toxic unit for humans – cancerogenic”, “Potential comparative toxic unit for humans - not cancerogenic”,
“potential soil quality index”. The results of this environmental impact indicator shall be used with care as the uncertainties on these
results are high as there is limited experience with the indicator.
This EPD was created using a software tool.
6. LCA: Interpretation
The manufacturing process (module A3), in particular the weight of the products. The impact of the raw materials is less
energy consumption, has the largest contribution on all impact significant. There are no benefits and loads from the end of life
categories. Besides the manufacturing, also the transport to the of the product, because the product is 100 % landfilled.
installation site (A4) has a significant contribution, due to the
7. Requisite evidence
8. References
Standards assessment – Principles and framework
EN 997 ISO 14044
WC pans and WC suites with integral trap - constructional and ISO 14044:2006: Environmental management – Life cycle
performance requirements. assessment – Requirements and guidelines.
EN 14688 ISO 45001
Sanitary appliances. Wash basins. Functional requirements and ISO 45001:2018: Occupational health and safety management
test methods systems Requirements with guidance for use
EN15804 PCR Part A
EN15804:2012+A2:2019+AC:2021, Sustainability of Calculation rules for the Life Cycle Assessment and
construction works — Environmental Product Declarations — Requirements on the Background Report, Institut Bauen und
Core rules for the product category of construction products. Umwelt e.V., www.bauumwelt.com.
ISO 9001 PCR Part B
ISO 9001:2015: Quality management systems — Requirements Institut Bauen und Umwelt e.V, Berlin (pub.): PCR Guidance-
Texts for Building-Related Products and Services From the
ISO 14001 range of Environmental Product Declarations of Institute
ISO 14001:2015: Environmental management systems — Construction and Environment e.V. (IBU) : Requirements on the
Requirements with guidance for use EPD for Toilet set
ISO 14025 Further references
EN ISO 14025:2011, Environmental labels and declarations —
Type III environmental declarations — Principles and CPR
procedures. European Regulation N° 305/2011 (CPR)
ISO 14040 Ecoinvent
ISO 14040:2006: Environmental management – Life cycle Wernet, G., Bauer, C., Steubing, B., Reinhard, J., Moreno-Ruiz,
6 Environmental Product Declaration - Ideal Standard International - Ceramic Fine Fireclay ISI
E., and Weidema, B., 2016. The ecoinvent database version 3
(part I): overview and methodology. The International Journal of PEFCR
Life Cycle Assessment, [online] 21(9), pp.1218–1230. Available European commission (2018). Product Environmental Footprint
at:http://link.springer.com/10.1007/s11367-016-1087-8 Category Rules PEFCR Guidance, version 6.3.
IBU Pré Consultants (2021)
IBU 2021. Institut Bauen und Umwelt e.V.: General Instructions SimaPro 9.3.0.3 [Computer Software]. Amersfoort, The
for the EPD programme of Institut Bauen und Umwelt e.V., Netherlands.
Version 2.0, Berlin: Institut Bauen und Umwelt e.V., 2021
www.ibu-epd.com REACH candidate list
ECHA, REACH Candidate List of substances of very
Industry 2.0 highconcern for Au Biocide Products No. 528/2012 EU,
Industry 2.0 (from PlasticsEurope, worldsteel and ERASM) LCA REGULATION (EU) No 528/2012 OF THE
database as integrated in SimaPro 9.3.0.3. EUROPEANPARLIAMENT
7 Environmental Product Declaration - Ideal Standard International - Ceramic Fine Fireclay ISI
Publisher
Institut Bauen und Umwelt e.V. +49 (0)30 3087748- 0
Hegelplatz 1 info@ibu-epd.com
10117 Berlin www.ibu-epd.com
Germany
Programme holder
Institut Bauen und Umwelt e.V. +49 (0)30 3087748- 0
Hegelplatz 1 info@ibu-epd.com
10117 Berlin www.ibu-epd.com
Germany
Author of the Life Cycle Assessment
Owner of the Declaration
Ideal standard International +33622608444
Da Vincilaan 2 eboukari@idealstandard.com
1935 Zaventem Belgium www.idealstandard.com
France
8 Environmental Product Declaration - Ideal Standard International - Ceramic Fine Fireclay ISI
