ENVIRONMENTAL PRODUCT DECLARATION
as per ISO 14025 and EN 15804+A1
Owner of the Declaration thomas gruppe - Geschäftsfeld Betonbauteile
Programme holder Institut Bauen und Umwelt e.V. (IBU)
Publisher Institut Bauen und Umwelt e.V. (IBU)
Declaration number EPD-THO-20200087-IBD1-EN
Issue date 24.08.2020
Valid to 23.08.2025
Floor plates
thomas betonbauteile
www.ibu-epd.com | https://epd-online.com
Umwelt Produktdeklaration Name des Herstellers – Name des Produkts
1. General Information
thomas betonbauteile Floor plates
Programme holder Owner of the declaration
IBU – Institut Bauen und Umwelt e.V. thomas gruppe - Geschäftsfeld Betonbauteile
Panoramastr. 1
10178 Berlin thomas beteiligungen GmbH
Germany Im Industriepark 13
55469 Simmern
Declaration number Declared product / declared unit
EPD-THO-20200087-IBD1-EN 1 t Floor plates
This declaration is based on the product Scope:
category rules: This document refers to Floor plates of the concrete
Pre-cast concrete components, 07.2014 components business area of the thomas group,
(PCR checked and approved by the SVR) produced in 1 out of 29 locatios:
Issue date thomas betonbauteile Rostock GmbH
24.08.2020 Werkstr. 8
18069 Rostock
Valid to
23.08.2025 The declared unit is 1 t of floor plates. The data for the
production of the declared product was collected on a
plant-specific basis with current annual data from 2018.
The declarant is responsible for the underlying data
and their verification.
The owner of the declaration shall be liable for the
underlying information and evidence; the IBU shall not
be liable with respect to manufacturer information, life
cycle assessment data and evidences.
The EPD was created according to the specifications
of EN 15804+A1. In the following, the standard will be
simplified as EN 15804.
Verification
The standard EN 15804 serves as the core PCR
Independent verification of the declaration and data
according to ISO 14025:2010
Dipl. Ing. Hans Peters internally x externally
(chairman of Institut Bauen und Umwelt e.V.)
Dr. Alexander Röder Angela Schindler
(Managing Director Institut Bauen und Umwelt e.V.)) (Independent verifier appointed by SVR)
2. Product
2.1 Product description/Product definition marking. For the application and use the respective
Floor plates are manufactured in the automatic national provisions apply.
circulation systems of the precasted concrete
plants. Floor plates consist of prefabricated reinforced 2.2 Application
concrete slabs and are supplemented by in-situ Floor plates of the thomas group from the concrete
concrete. They are used as ceiling elements in components business area are used in prefabricated
prefabricated buildings and differ in their size. buildings. They are applicable as load-bearing ceilings,
storey ceilings of buildings, parking and traffic areas as
For the placing on the market of the product in the well as covers.
European Union/European Free Trade Association
(EU/EFTA) (with the exception of Switzerland) 2.3 Technical Data
Regulation (EU) No. 305/2011 (CPR) applies. The The following technical data apply to floor plates. The
product needs a declaration of performance taking into standard EN 13747:2010, applies.
consideration EN 13747, 2010, Precast concrete
products - Floor plates for floor systems, and the CE-
2 Environmental Product Declaration thomas gruppe – Floor plates
Constructional data 2.6 Manufacture
Name Value Unit Shaping
Concrete Compressive The preliminary products such as aggregates, cement
fck ≥ C25/30
Strength and reinforced steel for the floor plates are delivered.
Tensile strength reinforcing The concrete is mixed together according to
ftk = 550 N/mm2
steel predefined recipes. Before casting the floor plates, the
Prestressing steel stress fpk N/mm2 formwork is created with the desired dimensions. The
Yield strength of reinforcing reinforcing bars for the reinforced concrete slabs are
fyk = 500 N/mm²
steel attached and then filled with concrete.
0.1% yield strength
Fp0,1 k N/mm²
prestressing steel Curing and Outplacement
measurement The floor plates are cured for 8-10 hours in drying
specification, chambers. After curing, they can be removed and can
Mechanical consistence harmonized acc. to be loaded. The standard strength is reached after 28
EN 13747:2005 + days after production.
AC:2006
measurement 2.7 Environment and health during
specification, manufacturing
Fire resistance (for the load harmonized acc. to Throughout the manufacturing process, additional
capacity) EN 13747:2005 + measures for health safety - exceeding the legal
AC:2006 measures for occupational safety for business
enterprises - are not required.
measurement
Hazards to water, air and soil can be excluded if the
specification,
product is used as intended. Corresponding to the
Corrsosion resistance harmonized acc. to
intended use of the construction products, no health
EN 13747:2005 +
impairments are known due to the raw materials
AC:2006
used.At the manufacturing location, certificates of the
Gross density 2.533 t/m³
environmental management systems EN 14001 exist.
2.8 Product processing/Installation
Performance data of the product in accordance with
For the installation, the generally valid laying
the declaration of performance with respect to its
instructions of the Fachvereinigung Betonbauteile mit
essential characteristics according to EN 13747, 2010,
Gitterträgern (Association for concrete components
Precast concrete products - Floor plates for floor
with lattice girders) for floor plates must be
systems.
observed. Floor plates are unloaded from the truck
with the construction site crane or mobile crane and
2.4 Delivery status
laid within the same operation.
For safety reasons and to avoid damage during
transport floor plates can be loaded on pallets. The
2.9 Packaging
dimensions of the floor plates are:
Floor plates are stacked and ransported to the
construction site by truck. For protection against
 Width: up to 2,5 m
damanges, stacking wood is placed between the
 Length up to 9 m
panels.
 Thickness: up to 8 cm
2.10 Condition of use
The floor plates are durable construction materials.
2.5 Base materials/Ancillary materials
The material composition does not change during
The main constituents of floor plates are:
service life.
 Cement: ca. 15 M.-%
2.11 Environment and health during use
 Ingredients: 75 - 80 M.-%
There are no known interactions between the product,
 Steel: < 5 M.-% the environment and health. Hazards for air and soil
 Water: 6 M.-% can be excluded if the described products are used as
intended.
This product or at least one partial article contains
2.12 Reference service life
substances listed in the candidate list (27.06.2018)
Based on the useful lives of building components
exceeding 0.1 percentage by mass: no.
according to the Sustainable Building Assessment
System BBSR, Service Lives of components for life
This product or at least one partial article contains
cycle assessment according to Assessment System for
other CMR substances in categories 1A or 1B which
are not on the ECHA candidate list, exceeding 0.1
percentage by mass: no.
Sustainable Building (BNB), the reference service life
Biocide products were added to this construction
of metal ceilings exceeds 50 years.
product or it has been treated with biocide products
(this then concerns a treated product as defined by the
(EU) Ordinance on Biocide Products No. 528/2012):
2.13 Extraordinary effects
no.
Fire
3 Environmental Product Declaration thomas gruppe – Floor plates
Floor plates declared here correspond to the class A1 engineering, road construction or e.g. for noise
of building products regarding their fire performance, barriers.
according to EN 13501-1. The steel scrap is collected and sent either directly or
via the scrap metal trade to secondary smelting
Fire protection companies. Floor plates can be refurbished to new
Name Value building products with comparatively little effort and
Building material class A1 energy.
Burning droplets -
Smoke gas development - 2.15 Disposal
Remains of floor plates and those from demolition
Water occurring on the construction site, can be disposed of
There are no known effects on the environment in the in accordance with the local regulations or Waste
event of unforeseen ingress of water. Classification Ordinance
(AVV) and the European Waste Catalogue (EWC). The
Mechanical destruction disposal code is 17 01 01 (concrete), if the recycling
In the case of mechanical destruction, floor plates may options mentioned above are not practical.
break.
2.16 Further information
2.14 Re-use phase Processing instructions, product data sheets, safety
Individual components of floor plates, such as concrete information and other technical information are
and steel, can be re-used after varietal segregation. available for download on the website of the thomas
Concrete can be ground and used as an additive in the group:
production of building materials as a secondary raw www.thomas-gruppe.de
material input, e.g. as filler and fill material in civil
3. LCA: Calculation rules
3.1 Declared Unit by estimates based on a medium transport distance of
The declaration applies to 1 t of floor plates. 300 km in Germany.
Floor plates vary in volume, mass and slightly in
composition. The average calculation is based on the 3.4 Cut-off criteria
average annual production. All relevant data, i.e. all applied materials according to
the recipe and the energy used originate from the
Declared unit production data acquisition and have been considered
Name Value Unit within the inventory analysis. Material- and
Declared unit 1 t energyflows with a proportion of less than 1 % were
Grammage 0.128 t/m² collected. It can be assumed, that the sum of the
Density 2533 t/m³ neglected processes does not exceed 5 % of the
Conversion factor to 1 kg 0.001 - impact categories.
.
3.5 Background data
Primary data has been provided by the manufacturer.
3.2 System boundary All background data required for the Life Cycle
The Life Cycle Assessment considers the system Assessment originates form the database
boundaries "cradle to grave" and follows the modular ÖKOBAUDAT 2019-III. Individual flows were
construction system described by EN 15804. The LCA complemented by ecoinvent 3.6 and GaBi ts 7.3.3.
takes into account the following
modules: 3.6 Data quality
The Life Cycle Assessment was essentially calculated
 A1: Raw material supply: extraction of raw based on result from impact assessments of upstream
activities. This leads to limitations on delared indicators
material, production of precursors, processing
(SM) and modules C3 and D.
of cement and aggregates, steel production,
For modelling the Life Cycle of floor plates, data has
casting and processing of recycling materials
been from the production year 2018. Background data
 A2: Transport of precursors: transport of raw has been taken from the various database. For the Life
materials to manufacturing plant Cycle Inventory all input and output flows have been
 A3: Manufacturing: production of floor plates respected.
 C1: De-Construction & Demolition of floor
3.7 Period under review
plates
The amount of raw materials, input energy and the
 C2: Transportation towards disposal volume of waste relate to the year 2018. It corresponds
 C4: Disposal of floor plates to the best currently available technology and thus is
representative for the considered time period. The
reference area is Germany.
3.3 Estimates and assumptions
3.8 Allocation
Plant and process specific data was provided for the
Co-product allocation does not exist in the
Life Cycle Assessment. Missing information on primary
manufacturing process.
data regarding transport distances were suplemented
4 Environmental Product Declaration thomas gruppe – Floor plates
3.9 Comparability
Basically, a comparison or an evaluation of EPD data
is only possible if all the data sets to be compared
were created according to EN 15804 and the building
context, respectively the product-specific
characteristics of performance, are taken into account.
The background data was used from various LCA
database. Thereby limitations on comparability of
EPDs may result.
The LCA background database ÖKOBAUDAT 2019-III
was used. Individual flows were complemented by
ecoinvent 3.6 and GaBi ts 7.3.3 .
4. LCA: Scenarios and additional technical information
The following technical information models the basisfor
the declared modules or can be used for developing
specific scenarios within the context of a building
assessment.
The reference life span according to ISO 15686-1
could not have been determined. The declaration of
the reference life span underlies the assessment
system of the Federal Institute for Research on
Building, Urban Affairs and Spatial Development
BBSR.
Reference service life
Name Value Unit
Reference service life (according
- a
to ISO 15686-1, -2, -7 and -8)
Life Span (according to BBSR) ≥ 50 a
End of life (C1-C4)
Name Value Unit
Landfilling 970 kg
Recycling 30 kg
5 Environmental Product Declaration thomas gruppe – Floor plates
5. LCA: Results
The table displayed below summarizes the results of the Life Cycle Assessment (LCA). The results of the impact
assessment do not provide any information on endpoints of the impact categories, exceedances of thresholds,
safety margins or risks. The results refer to the declared unit of 1 t floor plates. The Impact Assessment is based
on /CML 2001/ - April 2015. The Impact Assessment is based on CML 2001 - April 2015.
DESCRIPTION OF THE SYSTEM BOUNDARY (X = INCLUDED IN LCA; MND = MODULE NOT DECLARED;
MNR = MODULE NOT RELEVANT)
BENEFITS AND
CONSTRUCTI LOADS
PRODUCT STAGE ON PROCESS USE STAGE END OF LIFE STAGE BEYOND THE
STAGE SYSTEM
BOUNDARIES
6 Environmental Product Declaration thomas gruppe – Floor plates
lairetam
waR
ylppus tropsnarT
gnirutcafunaM
eht
morf
tropsnarT
etis
eht
ot
etag
ylbmessA esU
ecnanetniaM
riapeR
tnemecalpeR tnemhsibrufeR
ygrene
lanoitarepO esu
retaw
lanoitarepO esu
noitcurtsnoc-eD
noitilomed tropsnarT
gnissecorp
etsaW
lasopsiD -esueR -yrevoceR -gnilcyceR laitnetop
A1 A2 A3 A4 A5 B1 B2 B3 B4 B5 B6 B7 C1 C2 C3 C4 D
X X X MND MND MND MND MNR MNR MNR MND MND X X MND X MND
RESULTS OF THE LCA - ENVIRONMENTAL IMPACT according to EN 15804+A1: 1 t floor plates
Parameter Unit A1-A3 C1 C2 C4
Global warming potential [kg CO2-Eq.] 1.64E+2 8.63E-1 1.92E+0 1.44E+1
Depletion potential of the stratospheric ozone layer [kg CFC11-Eq.] 5.16E-7 2.84E-16 9.11E-16 8.47E-14
Acidification potential of land and water [kg SO2-Eq.] 1.89E-1 6.06E-4 4.33E-3 8.65E-2
Eutrophication potential [kg (PO4)3--Eq.] 4.59E-2 8.69E-5 1.06E-3 9.81E-3
Formation potential of tropospheric ozone photochemical
[kg ethene-Eq.] 1.92E-2 9.06E-5 -1.34E-3 6.64E-3
oxidants
Abiotic depletion potential for non-fossil resources [kg Sb-Eq.] 1.35E-4 3.02E-8 1.86E-7 5.32E-6
Abiotic depletion potential for fossil resources [MJ] 9.26E+2 1.18E+1 2.57E+1 2.02E+2
RESULTS OF THE LCA - RESOURCE USE according to EN 15804+A1: 1 t floor plates
Parameter Unit A1-A3 C1 C2 C4
Renewable primary energy as energy carrier [MJ] 2.22E+2 5.35E-2 1.61E+0 2.66E+1
Renewable primary energy resources as material utilization [MJ] 0.00E+0 0.00E+0 0.00E+0 0.00E+0
Total use of renewable primary energy resources [MJ] 2.22E+2 5.35E-2 1.61E+0 2.66E+1
Non-renewable primary energy as energy carrier [MJ] 1.01E+3 1.19E+1 2.58E+1 2.09E+2
Non-renewable primary energy as material utilization [MJ] 0.00E+0 0.00E+0 0.00E+0 0.00E+0
Total use of non-renewable primary energy resources [MJ] 1.01E+3 1.19E+1 2.58E+1 2.09E+2
Use of secondary material [kg] IND 0.00E+0 0.00E+0 0.00E+0
Use of renewable secondary fuels [MJ] 0.00E+0 0.00E+0 0.00E+0 0.00E+0
Use of non-renewable secondary fuels [MJ] 0.00E+0 0.00E+0 0.00E+0 0.00E+0
Use of net fresh water [m³] 3.60E-1 8.45E-5 1.82E-3 5.26E-2
RESULTS OF THE LCA – OUTPUT FLOWS AND WASTE CATEGORIES according to EN 15804+A1:
1 t floor plates
Parameter Unit A1-A3 C1 C2 C4
Hazardous waste disposed [kg] 3.35E-3 1.69E-9 1.46E-6 3.56E-6
Non-hazardous waste disposed [kg] 2.58E+1 1.51E-3 1.83E-3 9.71E+2
Radioactive waste disposed [kg] 3.04E-2 1.18E-5 3.90E-5 2.77E-3
Components for re-use [kg] 0.00E+0 0.00E+0 0.00E+0 0.00E+0
Materials for recycling [kg] 2.28E-1 0.00E+0 3.00E+1 0.00E+0
Materials for energy recovery [kg] 0.00E+0 0.00E+0 0.00E+0 0.00E+0
Exported electrical energy [MJ] 0.00E+0 0.00E+0 0.00E+0 0.00E+0
Exported thermal energy [MJ] 0.00E+0 0.00E+0 0.00E+0 0.00E+0
* MND: Modul not declared
6. LCA: Interpretation
The following figure shows the relative contributions of of the reinforcing steel in the product. The product
different Life Cycle processes and the primary energy considered in the model has a share of reinforcement
demand in the form of a dominance analysis. steel of 0.030 M% and has a greenhouse gas potential
(GWP) of 164 kgCO2e within production (A1–3). The
The Life Cycle Assessment was essentially calculated proportion of reinforcement steel can vary in individual
based on result from impact assessments of upstream cases (0.022 - 0.033 M%) and cause a range ofthe
activities. This leads to limitations on delared indicators greenhouse gas potential (GWP) within production
(SM) and modules C3 and D. (A1–3) of -1 % to +3 %.
Deviations in the material composition within the Unless otherwise stated, the fluctuations in all other
product may occur. The influence on the range of the impact categories are also small (<10 %).
environmental impact is determined by the proportion
Indicators of the impact assessment The negative POCP value for the transports is
explained by the methodical approach in calculating
The impact categories are determined throughout the the impact indicator: The negative POCP in the
life cycle mostly by module A1 (raw materials). The transports is caused by the division of the NOX
main driver is the use of cement, which contributes emissions into the two individual emissions NO2 and
about to 72 % to the greenhouse gas potential (GWP) NO. The NO has a negative influence on the POCP, as
in the production stage (A1–A3), followed by steel with it reduces the formation of ozone near the ground.
13 %. Contributions to the environmental impact from
the transport of the preliminary products (according to Abiotic depletion potential for non-fossil resources
the assumed scenario for A2) and the energy input for (ADP elem.)
production (A3) within the production stage are The ADP elem.-value is determined almost exclusively
comparable small. For the disposal of the construction by the provision of cement (92 %) and steel (5 %) at
waste (C1–C4) additional environmental burden the production stage. Electricity contributes for 1 % to
occurs. the ADP elem.-factor.
Global warming potential (GWP) Abiotic depletion potential for fossil resources
The global warming potential is mainly determined with (ADP foss.)
87% by the supply of raw materials: cement accounts Within the production stage (A1–A3), the ADP foss.-
for 72 % and steel for 13 %. The thermal energy value results mainly from high energy consumption
requirement and use of electricity contribute with 7 % required for the provision of cement and steel (approx.
to the GWP factor and the transport of preliminary 64 % in total). The use of electricity contributes for 4
products with approx. 6 %. %, fuel for 9 %.
Depletion potential of the stratospheric ozone layer Within the production (A1–3), the total primary
(ODP) energy demand is divided between approx. 82 %
The Ozone depletion potential is dominated almost nonrenewable energy sources and approx. 18 %
exclusively by the preliminary products (approx. 100 renewable energies.
%) and within them almost exclusively by the use of
cement. The use of electricity causes 100% of the Total use of non-renewable primary energy
ODP factor within manufacturing (A3). resources (PENRT)
The demand for non-renewable primary energy
Acidification potential of land and water (AP) resources result mainly for 71% from raw materials
The Acidification potential is determined by 54 % by (A1). The transport of the preliminary products (A2)
cement and 23 % by steel in the production stage. The contribute for 12 % and the production of the declared
use of energy sources in A3 contributes for 7 % to the product (A3) for 16 % to the PENRT value.
AP. With approx. 11 %, the transports have a minor For the disposal of the construction waste additional
influence on the acidification potential. use of non-renewable energy is due at the end of life.
In practice, different proportions of reinforcement are
Eutrophication potential (EP) used in the product (0.022 - 0.033 M%) and can cause
The Eutrophication potential is determined by 69 % by fluctuations in the non-renewable primary energy
cement and with 12 % by steel in the production stage. demand (PENRT) in the range of -6 % to + 2 % within
The use of energy sources in A3 contributes for 4 % to the production (A1–3).
the EP. With approx. 11 %, the transports have a
minor influence on the acidification potential. Total use of renewable primary energy resources
(PERT)
Potential of tropospheric ozone photochemical In comparison to the PENRT value the share of
oxidants (POCP) renewable resources is low. The majority of the PERT
About 82 % of the Photochemical oxidant potential is value is made up of raw material supply (A1) with 89
triggered by the use of cement and by the use of steel %, transportation 3% and the energy required for
(43 %). Due to different reinforcement components in production with approx. 7 %.
the product, the POCP factor can fluctuate by -10 % to For the disposal of the construction waste additional
+ 4 %. use of renewable energy is due at the end of life.
7 Environmental Product Declaration thomas gruppe – Floor plates
In practice, different proportions of reinforcement are
used in the product (0.022 - 0.033 M%) and can cause
fluctuations in the renewable primary energy demand
(PERT) within the production (A1–3) in the range from
-12 % to + 5 %.
7. Requisite evidence
Not relevant.
8. References
BBSR CMR Substances
Federal Institute for Research on Building, Urban European Chemical Agency (ECHA): CMR substances
Affairs and Spatial Development (BBSR): Service lifes from Annex VI of the CLP regulation registered under
of construction components. Service lifes of REACH and/ or notified under CLP.
construction components for Life Cycle Assessments
according to the assessment system for sustainable ÖKOBAUDAT 2019-III
construction (BNB), in: Federal Ministry for the Federal Ministry of the Interior, Building and
Environment, Nature Conservation, Building and Community (editor): Version 2019-III from 29.05.2019.
Nuclear Safety (ed.), 2017.
PCR A
Regulation 528/2012 Product category rules for building-related products
Regulation (EU) No 528/2012 of the European and service. Part A: Calculation rules for Life Cycle
Parliament and of the Council of 22 May 2012 Assessment and requirements on the project report,
concerning the making available on the market and version 1.7, 2018. Institut Bauen und Umwelt e.V.
use of biocidal products, in: Official Journal of the
European Union L 161/I, 2012. PCR B
PCR Guidance texts for building-related products and
Construction Product Regulation service. Part B: Requirements on the EPD for pre-cast
Construction Product Regulation (CPR): Regulation concrete components, version 1.7, 2019. Institut
(EU) No 305/2011 of the European Parliament and of Bauen und Umwelt e.V.
the Council of 9 March 2011 laying down harmonised
conditions for the marketing of construction products EN 1350-1
and repealing Council Directive 89/106/EEC (Text with EN13501-1: 2019, Fire classification of construction
EEA relevance), in: Official Journal of the European products and building elements - Part 1: Classification
Union, 2011. using data from reaction to fire tests.
CML 2001 EN 13747
Centrum voor Milieukunde der Universität Leiden, EN 13747:2010-08, Precast concrete products - Floor
Institute of Environmental Sciences, Leiden University, plates for floor systems.
The Netherlands: "Life Cycle Assessment. An
operational guide to the ISO standards, Volume 1, 2 EN 15804
and 3", 2001. EN 15804:2012-04+A1 2013, Sustainability of
construction works — Environmental Product
European Waste Catalogue Declarations — Core rules for the product category of
Waste Classification Ordinance (AVV)/ European construction products.
Waste Catalogue (EWC): Waste Classification.
Disposal Code 17 01 01 concrete. ISO 14025
DIN EN ISO 14025:2011-10, Environmental labels and
ecoinvent 3.6 declarations — Type III environmental declarations —
ecoinvent V. 3.6: Databank Version 3.6, Switzerland, Principles and procedures.
Dübendorf, [Access on 09.04.2019].
ISO 14001
Fachvereinigung Betonbauteile mit Gitterträgern ISO 14001: Environmental management systems -
Fachvereinigung Betonbauteile mit Gitterträgern e.V. Requirements with guidance for use.
(Hrsg.): Verlegeanleitung Elementdecken, 2012.
ISO15686-1
GaBi 7.3.3 ISO 15686-1:2011-05 Buildings and constructed
GaBi 7.3.3 databank edition, Thinkstep AG, 2017. assets - Service life planning - Part 1: General
principles and framewok.
Candidate List
European Chemical Agency (ECHA): Candidate List of
substances of very high concern for Authorisation, in:
https://echa.europa.eu/candidate-list-table, 2020.
8 Environmental Product Declaration thomas gruppe – Floor plates
Publisher
Institut Bauen und Umwelt e.V. Tel +49 (0)30 3087748- 0
Panoramastr. 1 Fax +49 (0)30 3087748- 29
10178 Berlin Mail info@ibu-epd.com
Germany Web www.ibu-epd.com
Programme holder
Institut Bauen und Umwelt e.V. Tel +49 (0)30 - 3087748- 0
Panoramastr 1 Fax +49 (0)30 – 3087748 - 29
10178 Berlin Mail info@ibu-epd.com
Germany Web www.ibu-epd.com
Author of the Life Cycle
Assessment Tel +49 7121 9223 50
myclimate Deutschland gGmbH Fax +49 7121 9223 8050
Borsigstraße 6 Mail kontakt@myclimate.de
72760 Reutlingen Web www.myclimate.de
Germany
Owner of the Declaration
thomas gruppe - Geschäftsfeld Tel +49 (6761) 901 100
Betonbauteile Fax +49 (6761) 901 101
Im Industriepark 13 Mail info@thomas-gruppe.de
55469 Simmern Web www.thomas-gruppe.de
Germany
