ENVIRONMENTAL PRODUCT DECLARATION
as per ISO 14025 and EN 15804+A2
Owner of the Declaration dormakaba International Holding GmbH
Publisher Institut Bauen und Umwelt e.V. (IBU)
Programme holder Institut Bauen und Umwelt e.V. (IBU)
Declaration number EPD-DOR-20210202-CBC1-EN
Issue date 19.01.2022
Valid to 18.01.2027
Panic and deadbolt locking device
dormakaba
www.ibu-epd.com | https://epd-online.com
General Information
dormakaba Panic and deadbolt locking device
Programme holder Owner of the declaration
IBU – Institut Bauen und Umwelt e.V. dormakaba International Holding GmbH
Hegelplatz 1 DORMA Platz 1
10117 Berlin 58256 Ennepetal
Germany Germany
Declaration number Declared product / declared unit
EPD-DOR-20210202-CBC1-EN 1 piece of the product: Panic and deadbolt locking device
This declaration is based on the product category rules: Scope:
Building Hardware products, 01.08.2021 This EPD refers to a specific product manufactured by dormakaba. The
(PCR checked and approved by the SVR) production site is located in Reamstown (USA).
The data represents the dormakaba financial year 2020/21.
Issue date The owner of the declaration shall be liable for the underlying information
and evidence; the IBU shall not be liable with respect to manufacturer
19.01.2022
information, life cycle assessment data and evidences.
The EPD was created according to the specifications of EN 15804+A2. In
Valid to
the following, the standard will be simplified as EN 15804.
18.01.2027
Verification
The standard EN 15804 serves as the core PCR
Independent verification of the declaration and data according to ISO
14025:2011
internally X externally
Dipl.-Ing. Hans Peters
(Chairman of Institut Bauen und Umwelt e.V.)
Florian Pronold Dr.-Ing. Wolfram Trinius,
(Managing Director Institut Bauen und Umwelt e.V.) (Independent verifier)
1 Environmental Product Declaration - dormakaba - Panic and deadbolt locking device
Product
Product description/Product definition Technical Data
This EPD report covers the Glass Pull (GP) Series panic and
deadbolt locking device.
GP Series panic and deadbolt locking device:
GP Series panic and deadbolt locking device accentuates glass
entrance doors with its sleek minimal tubular housing while
• For 3/8' through 7/8' glass doors
preserving a glass door's aesthetics. Versatile, durable, and
• Supports up to 120' tall doors
handsomely styled to accommodate sophisticated architectural
• +/- 1/2' adjustability height and width to accommodate
designs. dormakaba offers a complete glass exit device line
opening variances
manufactured on the east coast. The GP Series panic and
• 316 stainless steel
deadbolt locking device includes:
• Full range of exterior pull options
• Dogging functionality
Panic device
• Placeholder: Cylinder options/std.
• GP 1000 Series top latching bolt with manual and • 3-year warranty
electric strikes (fail safe or fail secure) The product with respect to its characteristics are in accordance
• GP 1100 Series bottom latching panic with manual with the relevant technical provisions (no CE-marking):
strikes
• Underwriter Laboratories (UL)
Deadbolt
• Americans with Disabilities Act (ADA)
• GP 1000 Series top locking deadbolt
• GP 1100 Series bottom locking deadbolt Base materials/Ancillary materials
• GP 1300 Series vertical deadbolt with top or bottom or The composition of the product is the following:
both top and bottom locking bolt options
• Interchangeable core cylinders or cylinder and
thumbturn
For the use and application of the product, the respective
national provisions at the place of use apply:
• ANSI/BHMA A156.3-2014, Grade 1
• UL305:2012
• ULC-S132-07:2016
Application
The product/s include/s partial articles which contain
The panic and deadbolt locking device can be used for:
substances listed in the Candidate List of REACH Regulation
• Entrances 1907/2006/EC (date: 19.01.2021) exceeding 0.1 percentage by
• Secure areas mass: No.
and following verticals:
Reference service life
• Commercial
The reference service life of the declared product is 10 years.
• Retail
This corresponds to approx.. 150.000 closing cycles per year,
• Hospitality
depending on the traffic pattern and frequency of usage.
• Entertainment
• Education
LCA: Calculation rules
The product stage includes:
Declared Unit — A1, raw material extraction, processing of secondary
The declared unit is 1 piece of the product: Panic device material input (e.g. recycling processes),
(GP1000, GP1100 and GP1300). — A2, transport to the manufacturer,
Declared unit — A3, manufacturing and assembly, processing and
mechanical treatments, including provision of all materials,
Name Value Unit
products and energy, as well as waste processing up to the
Declared unit 1 piece/product
end-of waste state.
Weight of declared unit 12.92 kg
Conversion factor to 1 kg (kg per declared Construction stage - Modules A4-A5
12.92 -
unit) The construction process stage includes:
— A4, transport to the building site;
System boundary — A5, treatment of waste packaging materials arising during
installation into the building.
The type of EPD is according to EN 15804: "cradle to gate with
options, modules C1–C4, and module D".
End-of-life stage– Modules C1-C4 and D
The following modules are declared: A1-A3, C, D and additional
The end-of-life stage includes:
modules: A4 + A5
— C1, de-construction, demolition;
— C2, transport to waste processing;
Production - Module A1-A3
2 Environmental Product Declaration - dormakaba - Panic and deadbolt locking device
— C3, waste processing for reuse, recovery and/or recycling; manufactured, used or handled at the end of the product´s
— C4, disposal; including provision and all transport, provision lifespan: North America
of all materials, products and related energy and water use.
Comparability
Module D (Benefits and loads beyond the system boundary)
includes: Basically, a comparison or an evaluation of EPD data is only
— D, recycling potentials, expressed as net impacts and possible if all the data sets to be compared were created
benefits. according to EN 15804 and the building context, respectively
the product-specific characteristics of performance, are taken
Geographic Representativeness into account. Background database: GaBi, SP40
Land or region, in which the declared product system is
LCA: Scenarios and additional technical information
Installation into the building (A5)
Characteristic product properties of biogenic carbon
Name Value Unit
Information on describing the biogenic Carbon Content at
Waste packaging (wood) 25 kg
factory gate
Name ValueUnit Reference service life
Biogenic carbon content in product - kg Name Value Unit
C
Life Span according to the manufacturer 10 a
Biogenic carbon content in accompanying kg
9.07
packaging C End of life (C1-C4)
Note: 1 kg of biogenic carbon is equivalent to 44/12 kg of CO . Name Value Unit
2
Recycling 12.91 kg
Energy recovery 0.01 kg
The following technical scenario information is required for the Transportation to waste management 50 km
declared modules and optional for non-declared modules.
The product is disassembled in a recycling process.Material
Transport to the building site (A4)
recycling is then assumed for the metals. The plastic
Name Value Unit components are assumed to be incinerated with energy
Litres of fuel 0.105 l/100km recovery. Minor proportions of residues arising from the
recycling process are landfilled (1%). Region for the End of Life
Transport distance 100 km
is: Global.
Capacity utilisation (including empty runs) 55 %
Truck transport to the construction site declared for 100 km. If Reuse, recovery and/or recycling potentials (D), relevant
necessary, the transport distance can be adjusted at building scenario information
level. Collection rate is 100%
3 Environmental Product Declaration - dormakaba - Panic and deadbolt locking device
LCA: Results
DESCRIPTION OF THE SYSTEM BOUNDARY (X = INCLUDED IN LCA; MND = MODULE OR INDICATOR NOT DECLARED; MNR
= MODULE NOT RELEVANT)
Benefits and
Construction loads beyond
Product stage Use stage End of life stage
process stage the system
boundaries
la ire ta m w a Ry lp p u s tro p s n a rT g n iru tc a fu n a M e h t m o rf tro p s n a rTe tis e h t o t e ta g y lb m e s s A e s U e c n a n e tn ia M ria p e R tn e m e c a lp e R tn e m h s ib ru fe R y g re n e la n o ita re p Oe s u re ta w la n o ita re p Oe s u n o itc u rts n o c -e Dn o itilo m e d tro p s n a rT g n is s e c o rp e ts a W la s o p s iD -e s u e R-y re v o c e R-g n ilc y c e Rla itn e to p
A1 A2 A3 A4 A5 B1 B2 B3 B4 B5 B6 B7 C1 C2 C3 C4 D
X X X X X MND MND MNR MNR MNR MND MND X X X X X
RESULTS OF THE LCA - ENVIRONMENTAL IMPACT according to EN 15804+A2: 1 piece panic and deadbolt locking device
(GP1000, GP1100 and GP 1300)
Parameter Unit A1-A3 A4 A5 C1 C2 C3 C4 D
GWP-total kg CO 2 eq 6.95E+01 3.32E-01 4.07E+01 0 5.69E-02 2.8E-02 1.53E-03 -6.81E+01
GWP-fossil kg CO 2 eq 1.02E+02 3.17E-01 7.53E-01 0 5.44E-02 2.8E-02 1.52E-03 -6.81E+01
GWP-biogenic kg CO 2 eq -3.27E+01 1.47E-02 3.99E+01 0 2.52E-03 6.51E-07 5.18E-06 1.83E-01
GWP-luluc kg CO 2 eq 1.51E-01 7.54E-06 5.22E-04 0 1.3E-06 1.58E-06 4.37E-06 -1.04E-01
ODP kg CFC11 eq 3.21E-11 3.35E-17 5.94E-15 0 5.75E-18 1.41E-17 5.62E-18 -6.63E-11
AP mol H+ eq 5.75E-01 3.17E-04 6.83E-03 0 5.45E-05 4.98E-06 1.09E-05 -2.62E-01
EP-freshwater kg P eq 1.11E-04 6.78E-08 1.04E-06 0 1.16E-08 2.25E-09 2.61E-09 -6.34E-05
EP-marine kg N eq 8.71E-02 1.01E-04 1.94E-03 0 1.73E-05 1.12E-06 2.8E-06 -4.19E-02
EP-terrestrial mol N eq 9.5E-01 1.12E-03 2.79E-02 0 1.93E-04 2.27E-05 3.08E-05 -4.54E-01
kg NMVOC
POCP 2.61E-01 2.85E-04 5.34E-03 0 4.9E-05 3.11E-06 8.48E-06 -1.24E-01
eq
ADPE kg Sb eq 3.47E-03 9.51E-09 9.4E-08 0 1.63E-09 1.93E-10 1.36E-10 -1.66E-03
ADPF MJ 1.18E+03 4.5E+00 1.03E+01 0 7.72E-01 1.3E-02 1.99E-02 -9.11E+02
m3 world eq
WDP 3.11E+01 6.21E-04 4.47E+00 0 1.07E-04 2.86E-03 1.59E-04 -2.11E+01
deprived
GWP = Global warming potential; ODP = Depletion potential of the stratospheric ozone layer; AP = Acidification potential of land and water; EP =
Eutrophication potential; POCP = Formation potential of tropospheric ozone photochemical oxidants; ADPE = Abiotic depletion potential for non-fossil
resources; ADPF = Abiotic depletion potential for fossil resources; WDP = Water (user) deprivation potential)
RESULTS OF THE LCA - INDICATORS TO DESCRIBE RESOURCE USE according to EN 15804+A2: 1 piece panic and deadbolt
locking device (GP1000, GP1100 and GP 1300)
Parameter Unit A1-A3 A4 A5 C1 C2 C3 C4 D
PERE MJ 2.54E+02 1.42E-02 3.27E+02 0 2.43E-03 3.37E-03 2.61E-03 -2.27E+02
PERM MJ 3.25E+02 0 -3.25E+02 0 0 0 0 0
PERT MJ 5.79E+02 1.42E-02 1.93E+00 0 2.43E-03 3.37E-03 2.61E-03 -2.27E+02
PENRE MJ 1.18E+03 4.5E+00 1.03E+01 0 7.73E-01 4.42E-01 1.99E-02 -9.12E+02
PENRM MJ 4.29E-01 0 0 0 0 -4.29E-01 0 0
PENRT MJ 1.18E+03 4.5E+00 1.03E+01 0 7.73E-01 1.3E-02 1.99E-02 -9.12E+02
SM kg 5.75E+00 0 0 0 0 0 0 0
RSF MJ 0 0 0 0 0 0 0 0
NRSF MJ 0 0 0 0 0 0 0 0
FW m3 1.1E+00 2.54E-05 1.05E-01 0 4.37E-06 6.84E-05 5.02E-06 -9.16E-01
PERE = Use of renewable primary energy excluding renewable primary energy resources used as raw materials; PERM = Use of renewable primary
energy resources used as raw materials; PERT = Total use of renewable primary energy resources; PENRE = Use of non-renewable primary energy
excluding non-renewable primary energy resources used as raw materials; PENRM = Use of non-renewable primary energy resources used as raw
materials; PENRT = Total use of non-renewable primary energy resources; SM = Use of secondary material; RSF = Use of renewable secondary fuels;
NRSF = Use of non-renewable secondary fuels; FW = Use of net fresh water
RESULTS OF THE LCA – WASTE CATEGORIES AND OUTPUT FLOWS according to EN 15804+A2:
1 piece panic and deadbolt locking device (GP1000, GP1100 and GP 1300)
Parameter Unit A1-A3 A4 A5 C1 C2 C3 C4 D
HWD kg 5.96E-06 4.36E-10 1.24E-08 0 7.49E-11 4.94E-11 3.03E-10 -2.8E-07
NHWD kg 1.16E+01 4.6E-04 7.98E-01 0 7.9E-05 2.9E-03 1E-01 -6.91E+00
RWD kg 1.66E-02 4.83E-06 5.73E-04 0 8.29E-07 4.81E-07 2.27E-07 -3.29E-02
CRU kg 0 0 0 0 0 0 0 0
MFR kg 0 0 0 0 0 1.29E+01 0 0
MER kg 0 0 0 0 0 0 0 0
EEE MJ 0 0 5.66E+01 0 0 0 0 0
EET MJ 0 0 1.02E+02 0 0 0 0 0
4 Environmental Product Declaration - dormakaba - Panic and deadbolt locking device
HWD = Hazardous waste disposed; NHWD = Non-hazardous waste disposed; RWD = Radioactive waste disposed; CRU = Components for re-use;
MFR = Materials for recycling; MER = Materials for energy recovery; EEE = Exported electrical energy; EET = Exported thermal energy
RESULTS OF THE LCA – additional impact categories according to EN 15804+A2-optional:
1 piece panic and deadbolt locking device (GP1000, GP1100 and GP 1300)
Parameter Unit A1-A3 A4 A5 C1 C2 C3 C4 D
Disease
PM 1.51E-05 1.67E-09 4.63E-08 0 2.86E-10 6.35E-11 1.35E-10 -4.93E-06
incidence
IR kBq U235 eq 1.62E+00 6.9E-04 8.96E-02 0 1.18E-04 4.33E-05 2.33E-05 -5.79E+00
ETP-fw CTUe 5.53E+02 3.19E+00 4.86E+00 0 5.47E-01 4.86E-03 1.14E-02 -3.99E+02
HTP-c CTUh 1.51E-05 5.99E-11 3.73E-10 0 1.03E-11 4.21E-13 1.69E-12 -1E-07
HTP-nc CTUh 1.72E-06 2.56E-09 2.33E-08 0 4.4E-10 4.26E-11 1.86E-10 -6.13E-08
SQP SQP 4.41E+03 1.16E-02 2.85E+00 0 1.98E-03 3.88E-03 4.15E-03 -1.22E+02
PM = Potential incidence of disease due to PM emissions; IR = Potential Human exposure efficiency relative to U235; ETP-fw = Potential comparative
Toxic Unit for ecosystems; HTP-c = Potential comparative Toxic Unit for humans (cancerogenic); HTP-nc = Potential comparative Toxic Unit for humans
(not cancerogenic); SQP = Potential soil quality index
Disclaimer 1 – for the indicator “Potential Human exposure efficiency relative to U235”. This impact category deals mainly with the
eventual impact of low-dose ionizing radiation on human health of the nuclear fuel cycle. It does not consider effects due to possible
nuclear accidents, occupational exposure or radioactive waste disposal in underground facilities. Potential ionizing radiation from the
soil, radon and from some construction materials is also not measured by this indicator.
Disclaimer 2 – for the indicators “abiotic depletion potential for non-fossil resources”, “abiotic depletion potential for fossil resources”,
“water (user) deprivation potential, deprivation-weighted water consumption”, “potential comparative toxic unit for ecosystems”,
“potential comparative toxic unit for humans – cancerogenic”, “Potential comparative toxic unit for humans - not cancerogenic”,
“potential soil quality index”. The results of this environmental impact indicator shall be used with care as the uncertainties on these
results are high as there is limited experience with the indicator.
References
Standards
Americans with Disabilities Act
ANSI/BHMA A156.3-2014 https://www.ada.gov/.
Revision of ANSI/BHMA A156.3 – 2008
AMERICAN NATIONAL STANDARD FOR EXIT DEVICES. IBU 2021
Institut Bauen und Umwelt e.V.: General Instructions for the
EN 15804 EPDs programme of Institut Bauen und Umwelt e.V. Version
EN 15804:2019+A2, Sustainability of construction works — 2.0., Berlin: Institut Bauen und Umwelt e.V., 2021. www.ibu-
Environmental Product Declarations — Core rules for the epd.com.
product category of construction products.ISO 14025DIN EN
ISO 14025:2011-10, Environmental labels and declarations — GaBi ts software
Type III environmental declarations — Principles and Sphera Solutions GmbH Gabi Software System and Database
procedures. for Life Cycle Engineering 1992-2020 Version 10.0.0.71
University of Stuttgart Leinfelden-Echterdingen.
ISO 14025
DIN EN ISO 14025:2011-10, Environmental labels and GaBi ts documentation
declarations — Type III environmental declarations — GaBi life cycle inventory data documentation
Principles and procedures. (https://www.gabisoftware.com/support/gabi/gabidatabase-
2020-lci-documentation/).
Registration, Evaluation, Authorisation and Restriction of
Chemicals (REACH) PCR Part A
Regulation (EC) No 1907/2006 of the European Parliament and PCR – Part A: Calculation Rules for the Life Cycle Assessment
of the Council on the Registration, Evaluation, Authorisation and Requirements on the Project Report according to EN
and Restriction of Chemicals (REACH). 15804+A2:2019, Version 1.0, Institut Bauen und Umwelt e.V.,
www.ibu-epd.com.
UL 305:2012
UL Standard for Safety Panic Hardware. PCR Part B
PCR – Part B: Requirements on the EPD for Building
ULC-S132-07:2016 Hardware product, version 1.2, Institut Bauen und
STANDARD METHOD OF TESTS FOR EMERGENCY EXIT Umwelt e.V., www.ibu-epd.com, 2017.
AND EMERGENCY FIRE EXIT HARDWARE.
Underwriters Laboratories
Further References https://ulstandards.ul.com/.
5 Environmental Product Declaration - dormakaba - Panic and deadbolt locking device
Publisher
Institut Bauen und Umwelt e.V. +49 (0)30 3087748- 0
Hegelplatz 1 info@ibu-epd.com
10117 Berlin www.ibu-epd.com
Germany
Programme holder
Institut Bauen und Umwelt e.V. +49 (0)30 3087748- 0
Hegelplatz 1 info@ibu-epd.com
10117 Berlin www.ibu-epd.com
Germany
Author of the Life Cycle Assessment
Sphera Solutions GmbH +49 711 341817-0
Hauptstraße 111- 113 info@sphera.com
70771 Leinfelden-Echterdingen www.sphera.com
Germany
Owner of the Declaration
dormakaba International Holding GmbH +49 2333 793-0
DORMA Platz 1 info.de@dormakaba.com
58256 Ennepetal www.dormakaba.com
Germany
6 Environmental Product Declaration - dormakaba - Panic and deadbolt locking device
