ENVIRONMENTAL PRODUCT DECLARATION
as per ISO 14025 and EN 15804+A2
Owner of the Declaration Grundfos Holding A/S
Publisher Institut Bauen und Umwelt e.V. (IBU)
Programme holder Institut Bauen und Umwelt e.V. (IBU)
Declaration number EPD-GRU-20230077-CBC1-EN
Issue date 21.11.2023
Valid to 20.11.2028
MAGNA3 40-80/100 (Cast Iron)
Grundfos Holding A/S
www.ibu-epd.com | https://epd-online.com
General Information
Grundfos Holding A/S MAGNA3 40-80/100 (Cast Iron)
Programme holder Owner of the declaration
IBU – Institut Bauen und Umwelt e.V. Grundfos Holding A/S
Hegelplatz 1 Poul Due Jensens Vej 7
10117 Berlin 8850 Bjerringbro
Germany Denmark
Declaration number Declared product / declared unit
EPD-GRU-20230077-CBC1-EN 1 PCS. of MAGNA3 40-80/100 (Cast iron)
This declaration is based on the product category rules: Scope:
Pumps for liquids and liquids with solids, 01.08.2021 The declaration applies to 1 piece of MAGNA3 (Cast Iron) pump. The
(PCR checked and approved by the SVR) product is produced in Wahlstedt, Germany, and the life cycle assessment
is based on data collected at the production site.
Issue date Production has been modeled using annual production data from 2021.
21.11.2023
The declaration covers two different types of the MAGNA3 40- product
(80/100).
The owner of the declaration shall be liable for the underlying information
Valid to
and evidence; the IBU shall not be liable with respect to manufacturer
20.11.2028 information, life cycle assessment data and evidences.
The EPD was created according to the specifications of EN 15804+A2. In
the following, the standard will be simplified as EN 15804.
Verification
The standard EN 15804 serves as the core PCR
Independent verification of the declaration and data according to ISO
14025:2011
internally X externally
Dipl.-Ing. Hans Peters
(Chairman of Institut Bauen und Umwelt e.V.)
Florian Pronold Mrs Kim Allbury,
(Managing Director Institut Bauen und Umwelt e.V.) (Independent verifier)
1 Environmental Product Declaration - Grundfos Holding A/S - MAGNA3 40-80/100 (Cast Iron)
Product
Product description/Product definition
The Grundfos MAGNA3 The products are also
circulator pumps are designed for circulating liquids in heating identical in terms of packaging, distribution, reference service
systems, air life and
conditioning and cooling systems and domestic hot water end-of-life treatment.
systems. However, the
pump range can also be used in ground source heat pump
systems and solar
heating systems. The only thing that
differentiates the products from each other is the software
which controls how
the pump operates in the system in which it is installed, making
them fit for
different applications.
Hence, all life cycle modules are identical, except use
stage module B6, which will change, as the applied scenarios
The MAGNA3 pump is a for electricity
centrifugal pump powered by an electrical motor. It has a high- consumption changes. For the placing
performance on the market in the European Union/European Free Trade
neodymium magnet rotor which increases motor efficiency and Association (EU/EFTA) (with the exception of Switzerland) the
an insulation shell following
to reduce heat loss from the cast iron pump housing with legal provisions apply:
threaded connections.
Machinery
Directive (2006/42/EC)
The declaration covers Standard used: EN
two types of the MAGNA3 pump. They are grouped as shown 809:1998 + A1:2009.
below. The group
reference in the technical data and scenarios refers also to
these.
GROUP 1 - MAGNA3 40-80
GROUP 2 - MAGNA3 40-100 Radio Equipment
Directive (2014/53/EU)
Standards used:
EN 60335-1:2012/AC:2014 + A11:2014, EN 60335-2-51:2003 +
A1:2008 + A2:2012,
EN 62233:2008.
These are all the same EN 55014-1:2006
physical products and 100 % identical in terms of design, + A1:2009 + A2:2011, EN 55014-1:2017, EN 61000-6-2:2005,
dimensions and EN 61000-3-2:2014, EN
materials as well as supply chain and manufacturing processes, 61000-3-3:2013, ETSI EN 301 489-1 V2.2.0, ETSI EN 301 489-
i.e., all cradle 17 V3.2.0. ETSI EN
to gate processes (A1-A3). 300 328 V2.1.1
Electromagnetic
Compatibility (EMC) Directive (2014/30/EU)
2 Environmental Product Declaration - Grundfos Holding A/S - MAGNA3 40-80/100 (Cast Iron)
Standards used: provisions
EN 55014-1:2017, EN 55014-2:2015, apply.
EN
61000-3-2:2014/2019, EN 61000-6-2:2008/2019,
The pump is
EN designed for circulating liquids in the
61000-3-3:2013 A1:2019
following
systems:
RoHS Directive ·
2011/65/EU and 2015/863//EU heating systems
Standard: EN ·
50581:2012. domestic hot-water systems
·
air-conditioning and cooling systems
Ecodesign
Directive (2009/125/EC) ·
ground-source heat-pump systems
Commission
Regulation (EC) No: 641/2009 and ·
solar-heating systems
Commission
Regulation (EU) 622/2012 The pump is
suitable for thin, clean, non-aggressive and non-explosive
liquids, not
containing solid particles or fibres that may attack the pump
Standards used: mechanically or
EN 16297-1:2012, EN 16297-2:2012, EN 16297-3:2012. chemically. In heating systems, the water must meet the
requirements of
accepted standards on water quality in
heating systems. The pumps are also suitable for domestic hot-
water systems.
Technical Data
The performance
The CE marking takes data of the product according to the harmonized norms, based
into account the proof of conformity with the respective on the
harmonized norms based harmonization provisions above apply.
on the legal provisions above.
MAGNA3 pumps are not harmonized in accordance with the
CPR.
The relevant
Application technical specifications according to the PCR Part B are given
For the in
application and use the respective national the table below.
3 Environmental Product Declaration - Grundfos Holding A/S - MAGNA3 40-80/100 (Cast Iron)
10.06.2022) exceeding 0.1 percentage by mass: no
Characteristics
that are the same for all product groups are only given once.
Others are given The Wahlstedt production has been assessed and
individually for all two groups. certified as meeting the requirements in ISO 14001, ISO 50001,
ISO
Constructional data
45001 and ISO 9001.
Name Value Unit
Frequency 50 Hz Reference service life
Voltage 230 V No use stage
scenario which refers to the lifetime of the product is declared.
Clean
Pumped liquid (e.g. water) - However, to
Water
facilitate building calculations, an estimated RSL of 10 years
Energy Efficiency Index Gr.1 0,19
can be used.
Energy Efficiency Index Gr.2 0,18 This is an EU consensus-based estimation, referenced on page
Flow range Gr. 1 (max) 18,5 m3/h 37 in Appendix 7: Lot
Flow range Gr. 2 (max) 21,0 m3/h 11 – Circulators in Buildings, prepared by AEA Energy &
Environment for
Head max. Gr.1 8 m
the European Commission in the context of the Eco Design
Head max. Gr.2 10 m
Directive:
Power input Gr. 1 Average (from load profile
0,117 kW
describing use)
Power input Gr. 2 Average (from load profile
0,163 kW
describing use)
Nominal capacity Gr.1 0,267 kW
Nominal capacity Gr.2 0,359 kW
Performance There is no
data of the product according to the harmonized definitive information on the average circulator life available,
standards, based on provisions for harmonization. there is consensus
within the industry that it is at least 12 years. However, this is
Base materials/Ancillary materials
complicated by
Base materials / Ancillary materials many factors, including many being scrapped prematurely
when e.g. the
Name Value Unit
boiler they are connected to is replaced.
Aluminium 17 %
Cast iron 45 %
Ceramics 0,4 %
Copper 3 %
Electronics 0,3 %
Magnet Nd 1 %
Paper 1 %
From the
PCB 5 % estimated stock (140Mpa) and annual sales (14Mpa), the
Plastics 0,4 % average lifetime of
Plastics, foam 1 % the circulator is taken as 10 years for the purposes of this study.
Plastics GF 6 %
Rubber 0,2 %
Stainless steel 6 %
Steel 6 %
Cardboard 9 %
Plastic film 0,1 %
The RSL of the
TOTAL 100 %
declared product is not directly influencing the results in this
REACH study, as no
This product/article/at least one partial article declared use stage scenario is dependent on the RSL; The use
contains stage sub-module
B6 is declared per year as required by the PCR Part B.
substances listed in the ECHA candidate list (date:
4 Environmental Product Declaration - Grundfos Holding A/S - MAGNA3 40-80/100 (Cast Iron)
LCA: Calculation rules
Declared Unit processes that provide the material and energy inputs
The declared unit is 1 piece (pcs.) of MAGNA3 (Cast into the system and the following manufacturing, transport up to
iron) pump. the factory
Declared unit gate as well as the processing any waste arising from those
processes.
Name Value Unit
Declared unit 1 pce.
Mass reference 18.74 kg/pce
Conversion factor [Mass/Declared Unit] 18.74 Wastes and losses are included in the modules where
they occur according to the polluter pays principle and the
For IBU core EPDs (where clause 3.6 is part of the EPD): for
modular approach of
average EPDs, an estimate of the robustness of the LCA
EN 15804.
values must be made, e.g. concerning the variability of the
production process, geographical representativeness and the
influence of background data and preliminary products
compared to the environmental impacts caused by the actual
production.
System boundary
The product includes:
This EPD is Cradle-To-Grave. The system boundaries
· A1
of the EPD follow the modular approach in EN 15804.
Extraction and processing of raw materials;
By decision no. 20170712-n of the SVR, the modules B3, B4
and B5 are by
default declared as "MNR" (module not relevant).
· A1 Reuse
of products or materials from a previous product system;
· A1
Processing of secondary materials;
The product stage (A1-A3)
comprises raw material extraction and processing, transport
processes as well
as the manufacturing process. The final production and
· A1
assembly of the MAGNA3
Generation of electricity, steam and heat from primary energy
pump takes place at a Grundfos manufacturing site in
resources, also
Germany. However, the full
including their extraction, refining and transport;
supply-chain leading to the finished product at the gate is rather
complex and
includes a large amount of raw materials, components and
semi-finished parts
· A1 Energy
which comes from both external suppliers as well as other
recovery and other recovery processes from secondary fuels;
Grundfos production
facilities
· A2
Transportation up to the factory gate and internal transport;
· A3
Production of ancillary materials or pre products;
The product stage is included in the study, and
· A3 Manufacturing
according to EN 15804 the system boundary with nature is set
of products and coproducts;
to include
those
· A3
5 Environmental Product Declaration - Grundfos Holding A/S - MAGNA3 40-80/100 (Cast Iron)
Manufacturing of packaging; Consumption of electricity, thermal energy and water at
distribution center;
· A1-A3
processing up to the end-of-waste state or disposal of final ·
residues. Transportation from distribution center to construction site;
For secondary material inputs, the system boundary to · Wastage
the previous system (providing the secondary material) is set during distribution.
where outputs
reach the end-of-waste state. The recycling of secondary
material into new raw
materials is included in the system boundary of this study. A5:
Waste
·
materials from production processes that are recycled Installation process;
without any modification of the material's inherent
characteristics are modelled
as closed-loop within A1-A3. This is done up to the input mass
flow that was · Transport
used during production. of packaging waste to treatment site;
· Waste
treatment of packaging.
Waste for incineration arising in the product stage is
accounted for in the module where the waste is produced. The The packaging material does not reach the end of waste
environmental state but is incinerated as waste. According to European
loads from the incineration process are declared in the module statistics, the
where it occurs average R1 value of incineration plants is > 0.6. Therefore, it is
and the electricity and heat which are produced from the assumed
incineration is
considered as closed-loop within A1-A3, as described in PCR
Part A,
5.5.1. The input of biogenic carbon from the production of that packaging material is treated thermally in an
packaging material is incineration plant with R1 > 0.6. The loads from the combustion
inventoried in A3. As required by PCR Part A, the process of
corresponding packaging are declared in module A5 and the resulting energy
end-of-life module of the packaging material, A5, is also benefits in module
declared and the
emissions of biogenic carbon are inventoried.
D, as required by the PCR Part A, 5.5.2.
The construction process stage (A4-A5) includes:
Use stage (B1-B7):
A4:
·
Transportation from factory gate to distribution center:
The use stage, related to the building fabric
includes:
·
6 Environmental Product Declaration - Grundfos Holding A/S - MAGNA3 40-80/100 (Cast Iron)
· B1, use or
application of the installed product;
Contributions to operational energy use during the use
stage (B6) come from the electricity consumption of the
product. The annual
· B2, electricity consumption is calculated by multiplying the average
maintenance. power input,
which is based on a defined load profile, with the annual
running hours.
For use stage (B6) European Average electricity grid mix has
The use stage related to the operation of the building been used. These
values are declared in the scenarios section.
includes:
· B6,
operational energy use; The End-of-Life stage (C1-C4)
includes all activities from when the product reaches the end of
its service
life and no longer provides any functionality and until all
· B7, materials and
operational water use. components are processed for
In this study, all use stage modules are assessed, reuse/recycling or disposed of.
though B1, B2 and B7 are assessed to be zero. By decision no.
20170712-n of the
SVR, the modules B3, B4 and B5 are by default declared as
"MNR" (module
not relevant). The modules include the provision and According to EN 15804 and the PCR Part A,
transport of all materials, products and related energy and the end-of-life stage includes:
water use, as well
as waste processing up to the end-of-waste state or disposal of
final residues
during the use stage. They also include all impacts and · C1
deconstruction of the product from the
aspects related to the losses during the use stage
(i.e. production, transport, and waste processing and disposal · building,
of the lost including initial on-site sorting of the
products and materials).
· materials;
· C2
Generally, the geographical coverage of the datasets transportation of the discarded product to a recycling site and
used matches the actual processes taking place. Meaning, that transportation
when modelling taking place in Grundfos Bjerringbro, the of waste to final disposal;
Danish electricity grid mix is used
in the model and thermal energy from natural gas. These are
generally
of very high quality with very good technological, temporal and · C3 waste
geographical processing, collection of waste fractions from the
representativeness. deconstruction and waste
processing of material flows intended for reuse, recycling and
energy recovery;
7 Environmental Product Declaration - Grundfos Holding A/S - MAGNA3 40-80/100 (Cast Iron)
· C4 waste
disposal including physical pretreatment and management of flows leaving the product system that have not been
the disposal site. allocated as co-products and that have passed the end-of-
waste state are
included in module D.
At the end of life, the MAGNA3 pump is manually
disassembled from the piping system in which it has been
installed. The
definition of the applied end-of-life scenario in this EPD follows
the
requirements in the
Contributions to module D comes from waste
incineration processes in A5 and C3 as well as material
recycling in C3. The
PCR Part A, 6.2 regarding complex products, specific fractions and net flows are shown in the scenarios
with a combination of recycling, thermal waste treatment and section.
landfilling. 100 %
of the material is considered in the end of life scenario as
required by the PCR.
An overall collection rate of 90 % has been assumed.
Comparability
Materials from which energy is recovered in an Basically, a comparison or an evaluation of EPD data
incineration process with an R1-value above 0.60 are in this is only possible if all the data sets to be compared were created
study included with according to EN
the environmental burdens from the incineration process 15804 and the building context, respectively the product-
inventoried in C3, the specific
recovered energy is declared as exported energy in C3 characteristics of performance, are taken into account.
and the energy benefits are declared in D. This
procedure is according to the PCR Part A, 5.5.6. C3 includes
the
mechanical separation of the product followed by a series of
sorting steps.
Metal fractions are recycled and plastics, cardboard and Geographic Representativeness
electronics are Land or region, in which the declared product system is
assumed incinerated with energy recovery. The residual manufactured, used or handled at the end of the product´s
fractions are landfilled lifespan: Europe
and declared in C4.
Comparability
Basically, a comparison or an evaluation of EPD data is only
possible if all the data sets to be compared were created
The specific amounts are shown in the scenarios
according to EN 15804 and the building context, respectively
the product-specific characteristics of performance, are taken
into account. Software and
databases used: GaBi ts
section.
9.2.1.68
Beyond system boundary (D):
(database schema 8007) Ecoinvent v3.5..
According to EN 15804 module D includes the reuse, recovery
and/or
recycling potentials, expressed as net impacts and benefits.
Any declared
benefits and loads from net
8 Environmental Product Declaration - Grundfos Holding A/S - MAGNA3 40-80/100 (Cast Iron)
LCA: Scenarios and additional technical information
An estimated
Characteristic product properties of biogenic carbon RSL of 10 years can be used to facilitate building calculations.
The biogenic This is an EU
carbon content quantifies the amount of biogenic carbon in a consensus-based estimation, referenced in Appendix 7: Lot 11
construction – Circulators in
product leaving the factory gate, and it will be separately Buildings, prepared by AEA Energy & Environment for the
declared for the European Commission
product and for any accompanying packaging, as required from in the context of the Eco Design Directive.
the PCR Part A.
Reference service life
The Carbon content of Cardboard and Paper is assumed to
0.46 kg C. Overall, Name Value Unit
there is an amount of 9 weight-% Carbon in the product leaving Life Span according to the manufacturer 10 a
the factory gate
and has to be considered Operational energy use (B6)
Name Value Unit
Electricity consumption, Group 1 585 kWh/a
Electricity consumption, Group 2 815 kWh/a
Average power input, Group 1 0,117 kW
Information on describing the biogenic Carbon Content at
Average power input, Group 2 0,163 kW
factory gate
Running hours (all groups) 5.000 h/a
Name ValueUnit
Biogenic carbon content in accompanying kg End of life (C1-C4)
0.74
packaging C Name Value Unit
Note: 1 kg of biogenic carbon is equivalent to 44/12 kg of CO2 Collected as mixed construction waste 17,03 kg
Transportation distance (C2) 500 km
Aluminium for recycling 2,8 kg
The following technical scenario information is required for the
Steel for recycling 8,44 kg
declared modules and optional for non-declared modules.
Modules for which no information is declared can be deleted; Copper for recycling 0,51 kg
additional information can also be listed if necessary. Stainless steel for recycling 0,91 kg
Plastics for incineration w/energy 0,031 kg
The following technical information is a basis for the declared
Electronics for incineration w/energy 0,81 kg
modules or can be used for developing specific scenarios in the
Landfilling 2,28 kg
context of a building assessment if modules are not declared
(MND).
Reuse, recovery and/or recycling potentials (D), relevant
scenario information
A5 is not declared including the disposal of the packaging
Name Value Unit
material on the construction site, the amounts of packaging
materials included in the LCA calculations must be declared as A5, incineration w/energy recov. (LDPE foil) 3,85 MJ
technical scenario information for Module A5. A5, incineration w/energy recov.
6,99 MJ
(Paper/Cardboard)
C3, steel for recycling (net amounts) -1,2 kg
Transport from the gate to the site (A4) C3, stainless steel for recycling (net amounts) 0,52 kg
Name Value Unit C3, aluminium for recycling (net amounts) -0,383 kg
Litres of fuel 0,0332 l/100km C3, copper for recycling (net amounts) 0,221 kg
Transport distance 2003 km C3, plastics for incineration, w/ energy recov. 1,28 kg
Capacity utilisation (including empty runs) 85 % C3, electronics for incineration, w/ energy recov. 0,814 kg
Gross density of products transported 360 kg/m3
Wastage during distribution 0,02 %
Installation into the building (A5)
Name ValueUnit
Packaging waste for incineration (LDPE film) 0,031 kg
Packaging waste for incineration
1,72 kg
(Paper/Cardboard)
9 Environmental Product Declaration - Grundfos Holding A/S - MAGNA3 40-80/100 (Cast Iron)
LCA: Results
Characterization model: EN 15804 - 2012+A2 -
2019, PEF. By Decision no. 20170712-n of the IBU SVR, the modules B3, B4, B5
are marked as MNR (module not relevant) as default. The LCA results in module
B6 are given on a period of one year, according to PCR Part B. To obtain
the results from module B6 over the entire life cycle, the LCA results of
module B6 must be multiplied by the estimated RSL of 10 years. The
indicator results for module B6 are declared for Group 1. B6 indicator results
for other groups can be derived by multiplying the B6 indicator results with
the following factors:
Group 2: 1,39
DESCRIPTION OF THE SYSTEM BOUNDARY (X = INCLUDED IN LCA; MND = MODULE OR INDICATOR NOT DECLARED; MNR
= MODULE NOT RELEVANT)
Benefits and
Construction loads beyond
Product stage Use stage End of life stage
process stage the system
boundaries
la ire ta m w a Ry lp p u s tro p s n a rT g n iru tc a fu n a M e h t m o rf tro p s n a rTe tis e h t o t e ta g y lb m e s s A e s U e c n a n e tn ia M ria p e R tn e m e c a lp e R tn e m h s ib ru fe R y g re n e la n o ita re p Oe s u re ta w la n o ita re p Oe s u n o itc u rts n o c -e Dn o itilo m e d tro p s n a rT g n is s e c o rp e ts a W la s o p s iD -e s u e R-y re v o c e R-g n ilc y c e Rla itn e to p
A1 A2 A3 A4 A5 B1 B2 B3 B4 B5 B6 B7 C1 C2 C3 C4 D
X X X X X MND MND MNR MNR MNR X MND X X X X X
RESULTS OF THE LCA - ENVIRONMENTAL IMPACT according to EN 15804+A2: 1PCS of MAGNA3 40-80/100 (Cast Iron)
Parameter Unit A1 A2 A3 A4 A5 B6 C1 C2 C3 C4 D
GWP-total kg CO 2 eq 9.29E+01 1.17E+00 9.34E-01 1.17E+00 2.52E+00 2.37E+02 0 4.73E-01 5.85E+00 1.14E-01 -4.63E-01
GWP-fossil kg CO 2 eq 9.25E+01 1.17E+00 3.75E+00 1.17E+00 1.44E-01 2.35E+02 0 4.7E-01 5.84E+00 1.17E-01 -4.58E-01
GWP-
biogenic kg CO 2 eq 3E-01 -1.5E-03 -2.85E+00 -2.43E-03 2.37E+00 7.85E-01 0 -7.93E-04 5.08E-03 -3.53E-03 -2.31E-03
GWP-luluc kg CO 2 eq 1.4E-01 8.23E-03 3.5E-02 9.22E-03 8.56E-05 3.41E-01 0 3.83E-03 2.54E-03 1.03E-04 -2.58E-03
kg CFC11
ODP 9.16E-08 2.01E-16 4.06E-09 1.91E-11 4.62E-16 5.18E-12 0 8.67E-17 3.83E-14 2.64E-16 -7.55E-13
eq
AP mol H+ eq 5.4E-01 9.62E-03 1.41E-02 6.79E-03 7.23E-04 5.2E-01 0 2.78E-03 4.53E-03 3.64E-04 -1.23E-02
EP-
kg P eq 1.58E-03 3.13E-06 5.85E-05 3.8E-06 1.06E-07 6.29E-04 0 1.44E-06 6.74E-06 1.28E-05 -4.13E-06
freshwater
EP-marine kg N eq 6.64E-02 3.2E-03 2.97E-03 3.23E-03 2.64E-04 1.15E-01 0 1.34E-03 1.11E-03 8.4E-05 -6.03E-04
EP-terrestrial mol N eq 6.97E-01 3.54E-02 2.98E-02 3.58E-02 3.28E-03 1.21E+00 0 1.48E-02 1.26E-02 9.22E-04 -6.11E-03
kg NMVOC
POCP 2.05E-01 7.56E-03 8.49E-03 6.16E-03 6.89E-04 3.16E-01 0 2.54E-03 3.04E-03 2.7E-04 -2.03E-03
eq
ADPE kg Sb eq 5.58E-03 8.61E-08 5.22E-05 1.22E-06 7.69E-09 6.82E-05 0 3.82E-08 5.04E-07 7.93E-09 -6.17E-04
ADPF MJ 1.26E+03 1.54E+01 5.23E+01 1.57E+01 8.69E-01 4.14E+03 0 6.31E+00 3.13E+01 1.68E+00 -1.9E+01
m3 world eq
WDP 2.54E+01 1.02E-02 1.62E-01 1.72E-02 3.1E-01 5.13E+01 0 4.61E-03 8.01E-01 -1.3E-03 -3.8E-01
deprived
GWP = Global warming potential; ODP = Depletion potential of the stratospheric ozone layer; AP = Acidification potential of land and water; EP =
Eutrophication potential; POCP = Formation potential of tropospheric ozone photochemical oxidants; ADPE = Abiotic depletion potential for non-fossil
resources; ADPF = Abiotic depletion potential for fossil resources; WDP = Water (user) deprivation potential)
RESULTS OF THE LCA - INDICATORS TO DESCRIBE RESOURCE USE according to EN 15804+A2: 1PCS of MAGNA3 40-
80/100 (Cast Iron)
Parameter Unit A1 A2 A3 A4 A5 B6 C1 C2 C3 C4 D
PERE MJ 3.32E+02 7.9E-01 4.56E+01 9.82E-01 1.5E-01 1.83E+03 0 3.65E-01 1.35E+01 1.18E-01 5.52E+00
PERM MJ 0 0 0 0 0 0 0 0 0 0 ND
PERT MJ 3.32E+02 7.9E-01 4.56E+01 9.82E-01 1.5E-01 1.83E+03 0 3.65E-01 1.35E+01 1.18E-01 5.52E+00
PENRE MJ 1.26E+03 1.55E+01 5.23E+01 1.57E+01 8.7E-01 4.14E+03 0 6.33E+00 3.13E+01 1.68E+00 -1.88E+01
PENRM MJ 0 0 0 0 0 0 0 0 0 0 0
PENRT MJ 1.26E+03 1.55E+01 5.23E+01 1.57E+01 8.7E-01 4.14E+03 0 6.33E+00 3.13E+01 1.68E+00 -1.88E+01
SM kg 1.35E+01 0 2.31E-01 2.74E-03 0 0 0 0 0 0 0
RSF MJ 1.46E-23 0 0 2.91E-27 0 0 0 0 0 0 0
10 Environmental Product Declaration - Grundfos Holding A/S - MAGNA3 40-80/100 (Cast Iron)
NRSF MJ 1.71E-22 0 0 3.42E-26 0 0 0 0 0 0 0
FW m3 7.68E-01 9.25E-04 2.24E-02 1.22E-03 7.3E-03 2.12E+00 0 4.25E-04 2.55E-02 2.14E-05 2.59E-02
PERE = Use of renewable primary energy excluding renewable primary energy resources used as raw materials; PERM = Use of renewable primary
energy resources used as raw materials; PERT = Total use of renewable primary energy resources; PENRE = Use of non-renewable primary energy
excluding non-renewable primary energy resources used as raw materials; PENRM = Use of non-renewable primary energy resources used as raw
materials; PENRT = Total use of non-renewable primary energy resources; SM = Use of secondary material; RSF = Use of renewable secondary fuels;
NRSF = Use of non-renewable secondary fuels; FW = Use of net fresh water
RESULTS OF THE LCA – WASTE CATEGORIES AND OUTPUT FLOWS according to EN 15804+A2:
1PCS of MAGNA3 40-80/100 (Cast Iron)
Parameter Unit A1 A2 A3 A4 A5 B6 C1 C2 C3 C4 D
HWD kg 2.23E-04 6.3E-07 1.22E-04 7.71E-07 4.51E-09 1.71E-06 0 2.93E-07 1.62E-08 6.74E-09 -3.27E-04
NHWD kg 4E+00 2.35E-03 2.71E-01 3.45E-03 8.38E-02 2.94E+00 0 1E-03 5.49E-01 1.93E+00 1.45E+00
RWD kg 5.17E-02 2.35E-03 2.71E-01 3.45E-03 8.38E-02 2.94E+00 0 1E-03 5.49E-01 1.93E+00 1.45E+00
CRU kg 0 0 0 0 0 0 0 0 0 0 0
MFR kg 0 0 0 0 0 0 0 0 1.27E+01 0 0
MER kg 0 0 0 0 0 0 0 0 0 0 0
EEE MJ 0 0 0 0 3.85E+00 0 0 0 6.93E+00 0 0
EET MJ 0 0 0 0 6.99E+00 0 0 0 1.25E+01 0 0
HWD = Hazardous waste disposed; NHWD = Non-hazardous waste disposed; RWD = Radioactive waste disposed; CRU = Components for re-use;
MFR = Materials for recycling; MER = Materials for energy recovery; EEE = Exported electrical energy; EET = Exported thermal energy
RESULTS OF THE LCA – additional impact categories according to EN 15804+A2-optional:
1PCS of MAGNA3 40-80/100 (Cast Iron)
Parameter Unit A1 A2 A3 A4 A5 B6 C1 C2 C3 C4 D
Disease
PM 6.4E-06 1.21E-07 2.1E-07 4.05E-08 4.1E-09 4.36E-06 0 1.63E-08 3.84E-08 3.71E-09 -2.95E-07
incidence
IR kBq U235 eq 5.69E+00 4E-03 2.3E-01 5.98E-03 6.43E-03 1.03E+02 0 1.72E-03 7.57E-01 2.86E-03 -9.13E-02
ETP-fw CTUe 7.84E+02 1.15E+01 1.73E+01 1.15E+01 4.39E-01 1.77E+03 0 4.72E+00 1.37E+01 1.18E+00 -6.22E+00
HTP-c CTUh 1.66E-06 2.35E-10 6.46E-07 6.99E-10 2.16E-11 4.89E-08 0 9.77E-11 4.21E-10 6.79E-11 -6.88E-08
HTP-nc CTUh 2.35E-06 1.27E-08 5.21E-08 1.4E-08 1.02E-09 1.8E-06 0 5.6E-09 1.72E-08 5.92E-09 -5.1E-09
SQP SQP 3.53E+02 4.76E+00 8.54E+01 5.42E+00 2.36E-01 1.32E+03 0 2.21E+00 9.86E+00 1.22E-01 -1.48E+01
PM = Potential incidence of disease due to PM emissions; IR = Potential Human exposure efficiency relative to U235; ETP-fw = Potential comparative
Toxic Unit for ecosystems; HTP-c = Potential comparative Toxic Unit for humans (cancerogenic); HTP-nc = Potential comparative Toxic Unit for humans
(not cancerogenic); SQP = Potential soil quality index
Disclaimer
1 – for the indicator 'Potential Human exposure efficiency relative to U235'.
This impact category deals mainly with the eventual impact of low-dose ionizing
radiation on human health of the nuclear fuel cycle. It does not consider
effects due to possible nuclear accidents, occupational exposure or
radioactive waste disposal in underground facilities. Potential ionizing
radiation from the soil, radon and from some construction materials is
also not measured by this indicator.
Disclaimer 2 – for the
indicators 'abiotic depletion potential for non-fossil resources', 'abiotic
depletion potential for fossil resources', 'water (user) deprivation potential,
deprivation-weighted water consumption', 'potential comparative toxic unit for
ecosystems', 'potential comparative toxic unit for humans – cancerogenic',
'Potential comparative toxic unit for humans - not cancerogenic', 'potential
soil quality index'. The results of this environmental impact indicator shall
be used with care as the uncertainties on these results are high as there is
limited experience with the indicator.
Disclaimer 3: JRC
Technical Reports, Version 2, 2018 Page 6, for the
indicator "EP-freshwater". This indicator has been calculated as 'kg
P eq' as required in the characterization model EUTREND model, Struijs et al.,
11 Environmental Product Declaration - Grundfos Holding A/S - MAGNA3 40-80/100 (Cast Iron)
2009b, as implemented in ReCiPe; This EPD was created using a software tool.
References
Standards
2014 on the
harmonistion of the laws of the Member
Machinery States relating
Directive to electromagnetic compatibility
DIRECTIVE 2006/42/EC
OF THE EUROPEAN
Ecodesign
PARLIAMENT AND Directive
OF THE COUNCIL of 17 May
DIRECTIVE
2006 on 2009/125/EC OF THE EUROPEAN
machinery
PARLIAMENT AND
OF THE COUNCIL of 21 October
Radio Equipment 2009
Directive establishing a framework for the setting of
DIRECTIVE ecodesign
2014/53/EU OF THE EUROPEAN PARLIAMENT AND OF THE requirements for energy-related products
COUNCIL of 16 April 2014 on
the harmonisation of the laws of the Member States relating to
the making
available on the market of
radio equipment EC 641/2009
COMMISSION
REGULATION (EC) No 641/2009 of 22 July 2009 implementing
Directive 2005/32/EC
of the European Parliament and of the Council with regard to
Electromagnetic ecodesign
Compatibility (EMC) Directive requirements for glandless standalone circulators and
glandless circulators integrated
in
DIRECTIVE
2014/30/EU OF THE EUROPEAN
products
PARLIAMENT AND
OF THE COUNCIL of 26 February
12 Environmental Product Declaration - Grundfos Holding A/S - MAGNA3 40-80/100 (Cast Iron)
substances
EC 622/2012
COMMISSION
REGULATION (EU) No 622/2012 of 11 July 2012 amending ETSI EN 301
Regulation (EC) No 489-1
641/2009 with regard to ecodesign requirements for glandless
standalone
circulators and glandless circulators integrated in products
ETSI EN 301
489-1 V2.2.0, Electromagnetic Compatibility (EMC) standard for
radio equipment
and services; Part 1: Common technical requirements
DIRECTIVE
2011/65/EU
ETSI EN 301
DIRECTIVE 489-17
2011/65/EU OF THE EUROPEAN
ETSI EN 301
PARLIAMENT AND 489-17 V3.2.0, Electromagnetic Compatibility (EMC) standard
OF THE COUNCIL of 8 June 2011 for radio equipment
and services; Part 17: Specific conditions for Broadband Data
Transmission
Systems
on the
restriction of the use of certain hazardous
substances in
electrical and electronic equipment
DIRECTIVE
2015/863/EU ETSI EN 300 328
V2.1.1
DIRECTIVE
2015/863/EU of 31 March 2015 amending ETSI EN 300 328
V2.1.1, Wideband transmission systems; Data transmission
equipment operating in
the 2,4 GHz ISM band and using wide band modulation
Annex II to techniques
Directive 2011/65/EU of the European
Parliament and
of the Council as regards the list of
EN 809
restricted
13 Environmental Product Declaration - Grundfos Holding A/S - MAGNA3 40-80/100 (Cast Iron)
EN 809:1998-10
+ A1:2009, Pumps and pump units for
respect to the
restriction of hazardous substances
liquids -
Common safety requirements
EN 60335-1
EN 55014-1
EN
60335-1:2012/A11:2014/A13:2017, Household
EN
55014-1:2017, Electromagnetic compatibility – Requirements
for household and similar
appliances, electric tools and similar apparatus – Part 1: electrical appliances – Safety – Part 1:General requirements
Emission
EN 60335-2-51
EN 55014-2
EN
EN 60335-2-51:2003-03 + A1:2008 + A2:2012, Household and
55014-2:2015, Electromagnetic compatibility – similar electrical
appliances – Safety –Part 2-51: Particular requirements for
stationary
circulation pumps for heating and service water installations
Requirements
for household appliances, electric tools
and similar
apparatus – Part 2: Immunity – Product
EN 61000-3-2
family standard
(CISPR 14-2:2015) EN
61000-3-2:2014/2019, Electromagnetic compatibility (EMC) –
Part 3-2: Limits –
Limits for harmonic current emissions (equipment input current
=16 A per phase)
EN 50581:2012
EN 50581:2012, EN 61000-3-3
Technical documentation for the
EN
assessment of 61000-3-3:2013-08/ A1:2019, Electromagnetic compatibility
electrical and electronic products with (EMC) – Part 3-3:
14 Environmental Product Declaration - Grundfos Holding A/S - MAGNA3 40-80/100 (Cast Iron)
Limits – Limitation of voltage changes, voltage fluctuations and
flicker in public
low voltage supply systems, for equipment with
EN 16297-3
rated current
<= 16 A per phase and not subject to conditional connection
EN
16297-3:2012, Pumps – Rotodynamic pumps –Glandless
circulators – Part 3: Energy
efficiency index (EEI) for circulators integrated in products
EN 61000-6-2
EN ISO 14001
61000-6-2:2008/2019, Electromagnetic compatibility (EMC) –
Part 6-2: Generic
standards –Immunity for industrial environments
EN ISO
14001:2015-09, Environmental management systems -
Requirements with guidance
for use
EN 16297-1
EN ISO 14025
16297-1:2012-10, Pumps – Rotodynamic pumps –Glandless
circulators – Part 1:
General requirements and procedures for testing and
calculation of energy DIN EN /ISO
efficiency index (EEI) 14025:2011-10, Environmental labels and declarations — Type
III environmental
declarations — Principles and procedures
EN 15804
EN
15804:2012-04+A1 2013, Sustainability of construction works
— Environmental
Product Declarations — Core rules for the product category of
construction
products
EN 16297-2
EN 16297-2:2012-10,
Pumps – Rotodynamic pumps –Glandless circulators – Part 2:
Calculation of
energy efficiency index (EEI) for standalone circulators PCR Part A
15 Environmental Product Declaration - Grundfos Holding A/S - MAGNA3 40-80/100 (Cast Iron)
Institut Bauen
und Umwelt e.V., Berlin (pub.): Product Category Rules for
Building-Related
Products and Services, Product Category Rules for
Construction Products from
the range of Environmental Product Declarations of Institut
Bauen und Umwelt
(IBU), Part A: Calculation Rules for the Life Cycle Assessment CML 2001
and Requirements
on the Project Report, Version 1.7 (2021)
Impact
assessment characterization factors Institute of Environmental
Sciences, Leiden
University, Netherlands
PCR
Part B
Institut Bauen ECHA candidate
und Umwelt e.V., Berlin (pub.): Product Category Rules for list
Building-Related
Products and Services, Product Category Rules for
Construction Products from
the range of Environmental Product Declarations of Institut Candidate List
Bauen und Umwelt of substances of very high concern (SVHCs) for authorisation,
(IBU), Part B: Requirements on the EPD for Pumps for liquids European
and liquids with Chemicals Agency (ECHA), Helsinki, Finland
solids, Version 1.0 (2018)
Ecoinvent
Ecoinvent v3.5
GaBi ts
Further
references
GaBi ts 9.2.1.68
(database schema 8007)
CPR
REACH
REGULATION (EU)
No 305/2011 OF THE EUROPEAN PARLIAMENT AND OF
THE COUNCIL of 9 March 2011
laying down harmonised conditions for the marketing of Regulation (EC)
construction products No 1907/2006 of the European Parliament and of the Council of
and repealing Council Directive 89/106/EEC 18 December 2006
16 Environmental Product Declaration - Grundfos Holding A/S - MAGNA3 40-80/100 (Cast Iron)
concerning the Registration, Evaluation, Authorisation and
Restriction of
Chemicals (REACH) (Status: 27.06.2018)
Decision no.
20170712-n
SVR The literature referred to in the Environmental Product
Declaration must be listed in full.Standards already fully quoted
in the EPD do not need to be listed here again.
The current version of PCR Part A and PCR Part B of the PCR
Advisory Board document on which they are based must be referenced.
(formerly SVA)
17 Environmental Product Declaration - Grundfos Holding A/S - MAGNA3 40-80/100 (Cast Iron)
Publisher
Institut Bauen und Umwelt e.V. +49 (0)30 3087748- 0
Hegelplatz 1 info@ibu-epd.com
10117 Berlin www.ibu-epd.com
Germany
Programme holder
Institut Bauen und Umwelt e.V. +49 (0)30 3087748- 0
Hegelplatz 1 info@ibu-epd.com
10117 Berlin www.ibu-epd.com
Germany
Author of the Life Cycle Assessment
Grundfos Holding A/S +45 87501400
Poul Due Jensens Vej 7 atomic@grundfos.com
8850 Bjerringbro www.grundfos.com
Denmark
Owner of the Declaration
Grundfos Holding A/S +45 87501400
Poul Due Jensens Vej 7 atomic@grundfos.com
8850 Bjerringbro www.grundfos.com
Denmark
18 Environmental Product Declaration - Grundfos Holding A/S - MAGNA3 40-80/100 (Cast Iron)
