ENVIRONMENTAL PRODUCT DECLARATION
as per ISO 14025 and EN 15804+A2
Owner of the Declaration
Programme holder Institut Bauen und Umwelt e.V. (IBU)
Publisher Institut Bauen und Umwelt e.V. (IBU)
Declaration number EPD­HIL­20220118­IBA1­EN
Issue date 20.06.2022
Valid to 19.06.2027
Hilti HIT­HY 200­R V3
HILTI AG
www.ibu-epd.com | https://epd-online.com
Umwelt Produktdeklaration Name des Herstellers – Name des Produkts
1. General Information
HILTI AG HIT­HY 200­R V3
Programme holder Owner of the declaration
IBU – Institut Bauen und Umwelt e.V. Hilti AG
Hegelplatz 1 Feldkircher Str. 100
10117 Berlin FL­9494 Schaan
Germany Liechtenstein
Declaration number Declared product / declared unit
EPD­HIL­20220118­IBA1­EN The declared product is a HILTI injectable mortar HIT­
HY 200­R V3. The declared unit is one kilogram of
reaction resin product in the mixing ratio of the two
components necessary for processing. The packaging
is also included in the calculation. The declared unit is
stated in [kg].
This declaration is based on the product Scope:
category rules: This document refers to the injectable mortar HIT­HY
Reaction resin products, 11.2017 200­R V3 with its packaging. For the compilation of the
(PCR checked and approved by the SVR) life cycle assessment, specific data were collected
from the factory in Kaufering, Germany, of the HILTI
AG. Data from the year 2018 are used, which
Issue date
correspond to the annual average.
20.06.2022
The owner of the declaration shall be liable for the
Valid to
underlying information and evidence; the IBU shall not
19.06.2027
be liable with respect to manufacturer information, life
cycle assessment data and evidences.
The EPD was created according to the specifications
of EN 15804+A2. In the following, the standard will be
simplified as EN 15804.
The owner of the declaration shall be liable for the
underlying information and evidence; the IBU shall not
be liable with respect to manufacturer information, life
cycle assessment data and evidences.
The EPD was created according to the specifications
of EN 15804+A2. In the following, the standard will be
simplified as EN 15804.
Verification
The standard EN 15804 serves as the core PCR
Independent verification of the declaration and data
according to ISO 14025:2011
Dipl. Ing. Hans Peters internally x externally
(chairman of Institut Bauen und Umwelt e.V.)
Dr. Alexander Röder Matthias Klingler
(Managing Director Institut Bauen und Umwelt e.V.)) (Independent verifier)
2. Product
2.1 Product description/Product definition systems. During the curing phase, a very strong bond
is formed between the organic and inorganic binder
The declared product of HIT­HY 200­R V3 is a two­ matrix.
component system. The hybrid system formed during cement and resin
The resin component (component A) comprises a resin curing results in a cross­linked duromer with desired
based on methacrylate as well as mineral and cement­ design properties (high bond strengths within a short
like fillers. The curing agent component (component B) curing time) and particular long­term stability.
comprises of peroxide hardener, water and mineral Composite foils are used for the two­component foil
fillers. pack of HIT­HY 200­R V3. This kind of packaging
Mixing the two components A and B in the static mixer serves the following purposes: waste volume
initiates the curing (hardening) reaction of both binder
2 Environmental Product Declaration Hilti AG – HIT­HY 200­R V3
reduction, easy storage and transport, less packaging Hilti HIT-HY 200-R V3 displays the following
material. characteristics:
Through legislation and increased public awareness
users have increasingly become discerned towards the Performance data of the product in accordance with
use of styrene and other highly volatile components the declaration of performance with respect to its
with their resulting unpleasant odour and low flash essential characteristics according to
point (flammability). ETA 19/0665
The reaction resins used in all Hilti hybrid adhesives ETA 19/0600
contain no styrene, are practically odourless and have ETA 19/0601
a considerably higher flash point, i.e. higher than 100 ETA 20/0318
°C in comparison to 34 °C for styrene­based products. ETA-19/0632
HIT­HY 200­R V3 is the ultimate performance ICC ESR-4878
injectable hybrid mortar with approvals for rebar ICC ESR-4868
connections and heavy duty anchoring.
For the placing of the product on the market in the Shelf life of 12 months:
European Union European Free Trade Association Substrate temperature during installation ­10 to +40 °C
EU/EFTA) (with the exception of Switzerland) (internal method).
Regulation (EU) No. 305/2011 (CPR) applies. The
product needs a declaration of performance taking into Working time:
consideration the following European Technical ­10 to ­5 °C 180 min
Approvals > ­5 to 0 °C 90 min
ETA 19/0665 > 0 to +5 °C 45 min
ETA 19/0600 > 5 to +10 °C 30 min
ETA 19/0601 > 10 to +20 °C 15 min
ETA 20/0318 > 20 to +30 °C 9 min
ETA­19/0632 > 30 to +40 °C 6 min
and the CE­marking. For the application and use the
respective national provisions apply. Curing time:
­10 to ­5 °C 20 h
2.2 Application > ­5 to 0 °C 8 h
Hilti HIT­HY 200­R V3 serves for safely securing of > 0 to +5 °C 4 h
threaded rods and post­installed rebar connections in > 5 to +10 °C 150 min
cracked and uncracked concrete C20/25 to C50/60. > 10 to +20 °C 90 min
HIT­HY 200­R V3 is ETA approved for seismic C1 and > 20 to +30 °C 60 min
C2 category for anchoring and C1 category for rebar. It > 30 to +40 °C 60 min
also holds international code council (ICC) approvals
for static and A­F seismic designs. 2.4 Delivery status
The product Hilti HIT­HY 200­R V3 is available in foil­
Hilti HIT­HY 200­R V3 is a component of the Hilti packages with a total of 330 ml and 500 ml injectable
SAFEset concept. Hilti SAFEset is an approved mortar in the corresponding mixing ratio.
system which makes anchor installation an easier,
safer and faster process. It significantly improves the 2.5 Base materials/Ancillary materials
robustness of fastening and dramatically reduces the Hilti HIT­HY 200­R V3 is supplied in the form of a dual
possibilities of error during installation. As part of component film­wrapped pack comprising a resin
SAFEset HIT­HY 200­R V3 can be installed with component and a curing agent component at a volume
approved Hilti Hollow Drill bits and vacuum cleaners ratio of 5:1. The mixing ratio of resin and curing agent
that drill and clean the hole in one step for virtually components is automatically set during the injection
dust­free installation. When use with Hilti HIT­Z rod as process. Product curing commences directly after the
part of the SAFEset, no cleaning of the borehole is components are mixed.
required. The use of Hilti HDE­22 dispenser with
Volume Calculator app leads to no under or over fill, The product reviewed in this EPD contains the
reducing underfilling related risks and minimizing following component volumes:
mortar wastage.
Resin component:
2.3 Technical Data Methacrylate resin mixture: 30 to 40% by weight
Mineral fillers: 40 to 50% by weight
Cement: 10 to 20% by weight
Constructional data Other: < 5% by weight
Name Value Unit
Density EN ISO 1183­1 1830 kg/m3 Curing agent component:
Compressive strength Mineral fillers: 40 to 50% by weight
91 N/mm^2
(Tcure=120h) EN ISO 604 Aluminium oxide: 15 to 25% by weight
Elastic modulus (pressure) EN Water: 15 to 25% by weight
2700 N/mm^2
ISO 604 Dibenzoyl peroxide: 10 to 15% by weight
Tensile shear strength acc. to DIN not Other: < 5% by weight
N/mm2
EN 14293 relevant
Tensile bond strength acc. to DIN not This product article contains substances listed in the
N/mm2
EN 14293 relevant candidate list (date: 05.04.2022) exceeding 0.1
percentage by mass: no.
3 Environmental Product Declaration Hilti AG – HIT­HY 200­R V3
This product contains other CMR substances in
categories 1A or 1B which are not on the candidate
list, exceeding 0.1 percentage by mass: no.
Biocide products were added to this construction
product or it has been treated with biocide products
(this then concerns a treated product as defined by the
(EU) Ordinance on Biocide Products No. 528/2012):
no.
2.6 Manufacture
Most raw materials are sourced in Europe. The
transport is exclusively by truck for the European raw Illustration: Production process of the packaging
materials, and by truck and by ship for the others.
Chemical mortars are usually two­component systems 2.7 Environment and health during
consisting of a binder and a hardener. One of the base manufacturing
components of the binder is the reactive resin which in The manufacturing plant of HIT­HY 200­R V3,Hilti
the case of HIT­HY 200­R V3 is produced in Kaufering. GmbH Industriegesellschaft für Befestigungstechnik,
The resin production process is a chemical reaction of Hiltistr. 6, 86916 Kaufering, Germany, is certified
the corresponding educts to a basic resin with according to ISO 14001 which defines international
subsequent mixing of the basic resin with different standards for sustainable environmental management.
reactive diluents to a reactive resin. This process is The production site is also certified in accordance with
controlled and monitored by process control DIN EN ISO 50001 Energy Management Systems.
technology.
The production of chemical mortars consists of a 2.8 Product processing/Installation
mixing process and a filling process of the respective The product is delivered with Instructions for Use
single components (binder and hardener) and their explaining the basic steps for installation:
subsequent union to a two­component system
(packaging). Here as well process control technology 1) For safe handling the precautionary measures
is used to weigh and mix solid and liquid compounds described in the SDS (e.g. hand and eye protection)
according to the specification. In the next step both must be adhered to
well­mixed components run through an automized 2) Insert the cartridge into the red cassette
filling line in which each of the processed masses is 3) Screw on the mixing nozzle
filled into a tubular foil bag. Finally the single 4) Put the cassette into the dispenser system
components are combined in one packaging unit. The 5) Discard the first trigger pulls
two­pack foil bags are packed into cardboard boxes 6) Fill 2/3 of the borehole with mortar
and then finally shipped. The manufacturing plant of 7) Set the fixing element
HIT­HY 200­R V3, Hilti GmbH Industriegesellschaft für
Befestigungstechnik, Hiltistr. 6, 86916 Kaufering, After mixing the components and squeezing the mortar
Germany, is certified according to ISO 9001. The into the borehole the fixing element has to be set within
guideline defines international standards for quality the working time mentioned in Instructions for Use.
and process management. After the curing time, described as well in Instructions
The following flowcharts illustrate the underlying for Use, the mortar is ready to take up loads.
production process.
2.9 Packaging
Hilti HIT­HY 200­R V3 is supplied in the form of a 2­
foil­pack system and thus leads to very little waste
remaining after use on the construction site. After
curing, the product can be disposed of with household
waste. Full or only partially emptied cartridges must be
disposed of as special waste in accordance with official
regulations.
The outer packaging consisting of plastic foil and
cardboard boxes designed according to the product
size can be recycled. Packaging contaminated by the
product must be disposed in a safe manner in
accordance with local/national regulations.
For this EPD, the declared packaging is a weighted
meanvalue of all available packaging sizes. This
Illustration: Production process of the reaction results in a 120 g packaging composed of 58 g of
resin mixture plastic, 58g of paper and cardboard, 4 g of aluminium.
2.10 Condition of use
During the installation the temperature of the base
material must be between ­10°C and +40°C. The
temperature of the product should be between 5 ­ 25
°C during storage and 0 ­ 40°C during usage. Hilti
literature and official approvals must always be
considered. The two components of HIT­HY 200­R V3
4 Environmental Product Declaration Hilti AG – HIT­HY 200­R V3
are only for use in combination with the defined volume influence on the fire characteristics of a building
ratio and under the conditions mentioned above to structure in which they have been installed
build up a cross­linked filled duromer.
Fire protection
Name Value
2.11 Environment and health during use Building material class E/Efl
Refer to the Safety Data Sheet (SDS) for detailed No performence
Burning droplets
information on handling, storage as well as first aid, assessed
firefighting and accidental release measures and No performence
Smoke gas development
disposal considerations. Following the given assessed
instructions helps to minimize the risk for health and
environment. Water
The cured product is chemically inert and insoluble in
2.12 Reference service life water. HIT­HY 200­R V3 is certified for use as an
Hilti HIT­HY 200­R V3 is exposed to a wide variety of anchoring adhesive in concrete for water treatment
environmental factors during the use phase. The applications according to National Sanitation
anticipated Reference Service Life depends on the Foundation (US) /NSF/.
specific installation situation and the product exposure
scenario. The main factors influencing the period of Mechanical destruction
use involve weathering as well as mechanical loads It is recommended to use dust protection during
and chemical exposure. demolition of the cured chemical anchor.
2.14 Re-use phase
2.13 Extraordinary effects The product cannot be re­used. After usage the
product can be removed by demolition.
Fire
Even without any special fire safety features the 2.15 Disposal
Injection Systems comply with at least the Uncured Hilti HIT­HY 200­R V3 can be disposed of
requirements of the DIN EN 13501­1 standard for fire according to the European waste code 08 04 09* or 20
classes E and Efl. As cross­linked methacrylate resins 01 27*. The built­in cured anchor can be disposed as
do not melt or drip, the resins do not contribute construction waste for which the European waste code
towards spreading fire. Apart from the common 17 01 01 applies.
combustion produces carbon monoxide and carbon
dioxide, fire gases can contain traces of methyl 2.16 Further information
methacrylate, esters, alcohol, and hydrocarbons. Due Further information is available on request under
to the quantities used, they only have a subordinate anchor.hse@hilti.com and on the Hilti website:
www.hilti.group
3. LCA: Calculation rules
3.1 Declared Unit gas). Green electricity from wind turbines is
The declared product is a HILTI injection mortar HIT­ considered for the whole manufacturing process.
HY 200­R V3. The declared unit refers to one kilogram Production and transport of production losses, final
of reaction resin product in the required mixing ratio of product packaging and other inputs.
the two components. The packaging of 0,120 kg/kg of End­of­life of production waste (hazardous, non­
product is also included in the calculation. The hazardous and recyclable), production losses and raw
following table shows the data of the declared unit. material packaging, including waste and losses
transportation, processing and disposal.
Declared unit A4 – Transport (to construction site)
Name Value Unit Transportation of packaged products from the
Declared unit 1 kg manufacturing site to the construction site, including
potential in­betweens (retailer, workshop, etc.).
A5 – Installation­Construction
electricity consumption for drilling and
3.2 System boundary injectingElectricity consumption for injecting (in case of
The type of the EPD is cradle to grave. The following injection with electrical dispenser).
information modules are defined as system boundaries Production of the construction losses.
in this study: Provision and end­of­life of tools and accessories for
injectable mortars (manual or electrical dispenser with
A1 – Raw material supply: or without battery and with cartridge holder).
Production and packaging of the raw materials to be End­of­life of hazardous construction losses and
supplied to the manufacturer. All processes are packaging (uncured mortar and soiled packaging) and
included from cradle to gate. non­hazardous construction losses (cured mortar and
A2 – Transport (to manufacturing site): unsoiled packaging): including waste transportation,
Transportation of all the raw materials and their processing and disposal.
packaging between their production site and the C1 – Deconstruction/demolition
manufacturing site, for all transport modes (sea, road). Diesel for building demolition.
A3 – Manufacturing: C2 – Transport (to waste processing)
Production, supply and use of energy sources at the Transportation to waste processing facility.
manufacturing sites (electricity, biomass and natural C4– Waste disposal
5 Environmental Product Declaration Hilti AG – HIT­HY 200­R V3
Treatment and disposal of plastic to sanitary landfill. manufacture is less than 5% by weight and therefore
falls below the cut­off criterion of the total calculation.
For the environmental impact, the use of green
electricity (stage A3) was calculated taking into 3.5 Background data
account the residual electricity mix for the remaining The source for background data for the LCA
electricity. The proportion of the electricity demand calculations is the ecoinvent 3.8 database.
covered by green electricity in the total electricity
demand is 100%. 3.6 Data quality
For the compilation of the life cycle assessment,
3.3 Estimates and assumptions specific data were collected from the factory Kaufering,
In general, background data and elecricity mixes are in Germany, of the HILTI AG from the year 2018. The
chosen and calculated country­specifically for the background data from the ecoinvent 3.8 database
production processes. In some cases, assumptions used was updated in the year 2021 and thus of highly
were made because of a lack of primary or secondary up­to­date. The mass of the different components of
data, in particular for the following aspects: the reactive resin mixture come from the information in
 The synthesis way of raw materials which the recipe. The data quality is classified as appropriate.
were not available on the Ecoinvent database
3.7 Period under review
were used to reconstructed these material's
Data from the year 2018 are used, which correspond
impact
to the annual average.
 Some raw material's packaging composition
and transportation distances were estimated 3.8 Allocation
 The energy consumption for production of the The energy for manufacturing (A3) is supposed to be
current product (HIT­HY 200­R V3) was the same as for another HITLI product, which
consumptions were measured on production line. No
assimilated to the energy consumption
allocation was used for this stage.
measured on the production line of another
The used operating tools (stage A5), which are Hilti's
Hilti product, which has a very similar
manual or electrical dispenser can be used to inject the
manufacturing process HIT­HY 200­R V3 as well as other Hilti products. The
 Estimations were made to calculate the part of the dispenser's impact allocated to the current
energy consumption during installation product is based on the estimated total mass of
injected product each dispenser can be used for. This
 The transportation scenario to building site is
can be considered as a mass allocation.
based on french transportation companies
statistics.
3.9 Comparability
Basically, a comparison or an evaluation of EPD data
is only possible if all the data sets to be compared
3.4 Cut-off criteria were created according to EN 15804 and the building
All information modules considered were included in context, respectively the product­specific
the calculation in such detail that all requirements of characteristics of performance, are taken into account.
/EN 15804/ are met. The consumption of additional
inputs such as lubricants, oils or solvents used for The used background database is given by ecoinvent
3.8 database, to which this study refers.
4. LCA: Scenarios and additional technical information
Characteristic product properties Consumption when unloaded 0,25 L/km
Information on biogenic Carbon Consumption at fill capacity 0,38 L/km
The declared product contains 58 g of paper and Empty return rate 14 %
cardboard (outer packaging and user manual). Since Effective consumption 0,019 L/tkm
only this materials contain biogenic carbon, in addition
to a neglectable part contained in the raw materials' Installation into the building (A5)
packaging, all the biogenic carbon capture and release Name Value Unit
were cancelled to simplify the model. Electricity consumption 0.000279 kWh
The cancelled emission corresponds to 0,008 kg of Uncured mortar loss 0,04 kg
biogenic carbon (0,0279 kg of CO2) for a cancelled
Cured mortar loss 0,03 kg
capture of 0,014 kg of biogenic carbon (0,0521 kg of
Material loss 0.07 kg
CO2).
Hazardous waste (soiled
0,053 kg
packaging)
Non­hazardous waste (unsoiled
The following scenarios were considered for the LCA 0,067 kg
packaging)
calculations:
Transport to the building site (A4)
Name Value Unit
End of life (C1-C4)
Transport distance 900 km
Name Value Unit
lorry 16­32
Vehicle type ­ Fuel for building demolition 0,0437 MJ
metric ton
Distance to sanitary landfill 50 km
Effective load 21 t
Landfilling 1 kg
Maximum capacity 24 t
6 Environmental Product Declaration Hilti AG – HIT­HY 200­R V3
7 Environmental Product Declaration Hilti AG – HIT­HY 200­R V3
5. LCA: Results
DESCRIPTION OF THE SYSTEM BOUNDARY (X = INCLUDED IN LCA; ND = MODULE OR INDICATOR NOT
DECLARED; MNR = MODULE NOT RELEVANT)
BENEFITS AND
CONSTRUCTI LOADS
PRODUCT STAGE ON PROCESS USE STAGE END OF LIFE STAGE BEYOND THE
STAGE SYSTEM
BOUNDARIES
8 Environmental Product Declaration Hilti AG – HIT­HY 200­R V3
lairetam
waR
ylppus tropsnarT
gnirutcafunaM
eht
morf
tropsnarT
etis
eht
ot
etag
ylbmessA esU
ecnanetniaM
riapeR
tnemecalpeR tnemhsibrufeR
ygrene
lanoitarepO esu
retaw
lanoitarepO esu
noitcurtsnoc­eD
noitilomed tropsnarT
gnissecorp
etsaW
lasopsiD ­esueR ­yrevoceR ­gnilcyceR laitnetop
A1 A2 A3 A4 A5 B1 B2 B3 B4 B5 B6 B7 C1 C2 C3 C4 D
X X X X X ND ND MNR MNR MNR ND ND X X X X X
RESULTS OF THE LCA - ENVIRONMENTAL IMPACT according to EN 15804+A2: 1 kg HIT-HY 200-R V3
Core Indicator Unit A1 A2 A3 A4 A5 C1 C2 C3 C4 D
GWP­total [kg CO2­Eq.] 2.09E+0 4.88E­2 5.28E­1 6.98E­2 4.51E­1 4.02E­3 4.84E­3 0.00E+0 1.14E­1 0.00E+0
GWP­fossil [kg CO2­Eq.] 2.06E+0 4.87E­2 4.19E­1 6.95E­2 4.40E­1 4.02E­3 4.82E­3 0.00E+0 1.14E­1 0.00E+0
GWP­biogenic [kg CO2­Eq.] 2.99E­2 1.37E­4 1.08E­1 2.41E­4 1.08E­2 3.65E­6 1.67E­5 0.00E+0 2.85E­4 0.00E+0
GWP­luluc [kg CO2­Eq.] 1.34E­3 2.45E­5 7.89E­4 2.78E­5 2.38E­4 4.00E­7 1.93E­6 0.00E+0 2.15E­6 0.00E+0
ODP [kg CFC11­Eq.] 2.89E­7 1.09E­8 8.36E­8 1.61E­8 5.78E­8 8.59E­10 1.12E­9 0.00E+0 3.10E­9 0.00E+0
AP [mol H+­Eq.] 1.13E­2 4.01E­4 1.97E­3 1.97E­4 1.91E­3 4.17E­5 1.37E­5 0.00E+0 7.63E­5 0.00E+0
EP­freshwater [kg P4­Eq.] 6.27E­4 3.03E­6 1.37E­4 4.75E­6 1.33E­4 1.27E­7 3.30E­7 0.00E+0 8.58E­7 0.00E+0
EP­marine [kg N­Eq.] 2.31E­3 8.82E­5 4.99E­4 4.03E­5 3.29E­4 1.85E­5 2.79E­6 0.00E+0 2.14E­3 0.00E+0
EP­terrestrial [mol N­Eq.] 1.89E­2 9.76E­4 4.07E­3 4.38E­4 4.71E­3 2.03E­4 3.03E­5 0.00E+0 3.07E­4 0.00E+0
POCP [kg NMVOC­Eq.] 7.40E­3 2.87E­4 1.26E­3 1.68E­4 9.55E­4 5.57E­5 1.17E­5 0.00E+0 1.12E­4 0.00E+0
ADPE [kg Sb­Eq.] 2.53E­5 1.57E­7 1.76E­6 2.51E­7 6.36E­6 2.04E­9 1.74E­8 0.00E+0 3.11E­8 0.00E+0
ADPF [MJ] 3.54E+1 7.01E­1 7.67E+0 1.03E+0 4.62E+0 5.41E­2 7.17E­2 0.00E+0 2.22E­1 0.00E+0
[m³ world­Eq
WDP 1.74E+0 3.12E­3 1.92E­1 4.84E­3 1.86E­1 1.45E­4 3.36E­4 0.00E+0 2.30E­3 0.00E+0
deprived]
GWP = Global warming potential; ODP = Depletion potential of the stratospheric ozone layer; AP = Acidification potential of land and water; EP =
Caption Eutrophication potential; POCP = Formation potential of tropospheric ozone photochemical oxidants; ADPE = Abiotic depletion potential for non­
fossil resources; ADPF = Abiotic depletion potential for fossil resources; WDP = Water (user) deprivation potential
RESULTS OF THE LCA - INDICATORS TO DESCRIBE RESOURCE USE according to EN 15804+A2: 1 kg
HIT-HY 200-R V3
Indicator Unit A1 A2 A3 A4 A5 C1 C2 C3 C4 D
PERE [MJ] 1.69E+0 9.36E­3 6.86E­1 1.50E­2 2.39E­1 3.09E­4 1.04E­3 0.00E+0 1.17E­2 0.00E+0
PERM [MJ] 1.99E­3 0.00E+0 4.73E­1 0.00E+0 3.33E­2 0.00E+0 0.00E+0 0.00E+0 0.00E+0 0.00E+0
PERT [MJ] 1.69E+0 9.36E­3 1.16E+0 1.50E­2 2.73E­1 3.09E­4 1.04E­3 0.00E+0 1.17E­2 0.00E+0
PENRE [MJ] 2.53E+1 7.01E­1 5.25E+0 1.03E+0 3.70E+0 5.41E­2 7.17E­2 0.00E+0 2.22E­1 0.00E+0
PENRM [MJ] 1.01E+1 0.00E+0 2.43E+0 0.00E+0 9.19E­1 0.00E+0 0.00E+0 0.00E+0 0.00E+0 0.00E+0
PENRT [MJ] 3.54E+1 7.01E­1 7.68E+0 1.03E+0 4.62E+0 5.41E­2 7.17E­2 0.00E+0 2.22E­1 0.00E+0
SM [kg] 6.68E­3 2.66E­4 5.81E­2 3.52E­4 6.14E­3 2.12E­5 2.44E­5 0.00E+0 8.41E­5 0.00E+0
RSF [MJ] 1.37E­4 2.33E­6 4.83E­3 3.87E­6 3.74E­4 6.91E­8 2.69E­7 0.00E+0 3.83E­6 0.00E+0
NRSF [MJ] 0.00E+0 0.00E+0 0.00E+0 0.00E+0 0.00E+0 0.00E+0 0.00E+0 0.00E+0 0.00E+0 0.00E+0
FW [m³] 4.39E­2 8.25E­5 4.68E­3 1.32E­4 4.61E­3 3.28E­6 9.14E­6 0.00E+0 2.92E­4 0.00E+0
PERE = Use of renewable primary energy excluding renewable primary energy resources used as raw materials; PERM = Use of
renewable primary energy resources used as raw materials; PERT = Total use of renewable primary energy resources; PENRE = Use of
non­renewable primary energy excluding non­renewable primary energy resources used as raw materials; PENRM = Use of non­
Caption
renewable primary energy resources used as raw materials; PENRT = Total use of non­renewable primary energy resources; SM = Use
of secondary material; RSF = Use of renewable secondary fuels; NRSF = Use of non­renewable secondary fuels; FW = Use of net fresh
water
RESULTS OF THE LCA – WASTE CATEGORIES AND OUTPUT FLOWS according to EN 15804+A2:
1 kg HIT-HY 200-R V3
Indicator Unit A1 A2 A3 A4 A5 C1 C2 C3 C4 D
HWD [kg] 2.00E­1 8.56E­4 4.59E­2 1.18E­3 1.54E­1 7.23E­5 8.16E­5 0.00E+0 3.46E­4 0.00E+0
NHWD [kg] 2.32E+0 1.33E­2 4.98E­1 2.09E­2 3.47E­1 5.08E­4 1.45E­3 0.00E+0 1.00E+0 0.00E+0
RWD [kg] 5.80E­5 4.84E­6 1.30E­5 7.12E­6 1.36E­5 3.81E­7 4.93E­7 0.00E+0 1.47E­6 0.00E+0
CRU [kg] 0.00E+0 0.00E+0 0.00E+0 0.00E+0 0.00E+0 0.00E+0 0.00E+0 0.00E+0 0.00E+0 0.00E+0
MFR [kg] 1.51E­4 1.94E­5 3.37E­2 3.24E­6 7.46E­2 7.20E­8 2.25E­7 0.00E+0 1.21E­6 0.00E+0
MER [kg] 5.67E­6 1.80E­8 5.08E­7 2.61E­8 5.46E­7 1.15E­9 1.81E­9 0.00E+0 5.85E­9 0.00E+0
EEE [MJ] 1.39E­2 1.42E­4 9.61E­3 2.25E­4 2.55E­3 2.12E­5 1.56E­5 0.00E+0 4.53E­4 0.00E+0
EET [MJ] 5.62E­2 6.83E­4 2.94E­2 9.36E­4 9.26E­3 2.15E­4 6.49E­5 0.00E+0 1.22E­3 0.00E+0
HWD = Hazardous waste disposed; NHWD = Non­hazardous waste disposed; RWD = Radioactive waste disposed; CRU = Components
Caption for re­use; MFR = Materials for recycling; MER = Materials for energy recovery; EEE = Exported electrical energy; EEE = Exported
thermal energy
RESULTS OF THE LCA – additional impact categories according to EN 15804+A2-optional:
1 kg HIT-HY 200-R V3
Indicator Unit A1 A2 A3 A4 A5 C1 C2 C3 C4 D
[Disease
PM 9.90E­8 3.43E­9 2.22E­8 5.60E­9 1.85E­8 1.12E­9 3.88E­10 0.00E+0 1.62E­9 0.00E+0
Incidence]
[kBq U235­
IRP 1.55E­1 3.60E­3 3.25E­2 5.43E­3 2.39E­2 2.48E­4 3.76E­4 0.00E+0 1.48E­3 0.00E+0
Eq.]
ETP­fw [CTUe] 7.80E+1 5.63E­1 6.58E+0 8.63E­1 1.37E+1 3.25E­2 5.98E­2 0.00E+0 4.83E­1 0.00E+0
HTP­c [CTUh] 7.38E­9 2.18E­11 2.55E­10 2.65E­11 7.37E­10 1.25E­12 1.84E­12 0.00E+0 7.12E­12 0.00E+0
HTP­nc [CTUh] 1.07E­7 5.24E­10 5.06E­9 8.45E­10 1.06E­8 2.35E­11 5.86E­11 0.00E+0 1.81E­10 0.00E+0
SQP [­] 5.01E+0 4.26E­1 3.45E+0 7.35E­1 1.07E+0 7.03E­3 5.09E­2 0.00E+0 5.83E­1 0.00E+0
PM = Potential incidence of disease due to PM emissions; IR = Potential Human exposure efficiency relative to U235; ETP­fw = Potential
Caption comparative Toxic Unit for ecosystems; HTP­c = Potential comparative Toxic Unit for humans (cancerogenic); HTP­nc = Potential
comparative Toxic Unit for humans (not cancerogenic); SQP = Potential soil quality index
Disclaimer 1 – for the indicator “Potential Human exposure efficiency relative to U235”.
This impact category deals mainly with the eventual impact of low dose ionizing
radiation on human health of the nuclear fuel cycle. It does not consider effects due to possible
nuclear accidents, occupational exposure nor due to radioactive waste disposal in underground
facilities. Potential ionizing radiation from the soil, from radon and from some construction materials is also not
measured by this indicator.
Disclaimer 2 – for the indicators “abiotic depletion potential for non­fossil resources”, “abiotic depletion potential
for fossil resources”, “water (user) deprivation potential, deprivation­weighted water consumption”, “potential
comparative toxic unit for ecosystems”, “potential comparative toxic unit for humans – cancerogenic”, “Potential
comparative toxic unit for humans ­ not cancerogenic”, “potential soil quality index”.
The results of this environmental impact indicator shall be used with care as the
uncertainties on these results are high or as there is limited experienced with the indicator.
6. LCA: Interpretation
The dominance analysis shows that the main causes In the information module A1, the material supply of
of environmental impacts and indicators can be found the reaction resin mixture causes more than 80% of
in the information module A1. This shows the global the global warming potential.
warming potential for the provision of material with
more than 60%, based on all information modules.
Modules A3 and A5 also represent an import part of
the final impact
Illustration: Dominance analysis A1
The mass of the individual components of the reaction
resin mixture come from the recipe information
provided by the manufacturer. According to the
manufacturer, this information can be assumed to be
Illustration: Dominance analysis A1- C4 highly accurate.
Module A1 is detailed below. Module A3’s global The relevant datasets used to calculate the material
warming impact is mostly constituted by the final availability of the product are highly topical since the
product packaging (11% of the total impact) and raw materials were detailed as much as necessary to
energy for manufacturing (4% of the total impact). Most find corresponding data in the latest Ecoinvent
of the global warming impact from module A5 is database (2021). The locations were also respected.
caused by the product losses (6% of the final impact) Since these datasets strongly influence the results, as
the end­of­life of the soiled product packaging, treated shown by the dominance analysis, so does the overall
as hazardous waste (4% of the final impact). computation.
7. Requisite evidence
Hilti HIT­HY 200­R V3 complies with the requirements  emission class A+ outlined in the French VOC
of Directives (2019) in accordance with the
 DIBt (2010) in combination with the NIK
Eurofins attestation,
values from AgBB (2018) for applications in
 CDPH/EHLB Standard Method V 1.2 (2017)
interior areas,
9 Environmental Product Declaration Hilti AG – HIT­HY 200­R V3
in accordance with Eurofins test report, No. 392-2019- R (dimensionless) <1 ­
00435401_D_EN, Eurofins test report, No. 392-2019- VOC without NIK <100 μg/m3
00435401_E_EN and Eurofins test report, No. 392- Carcinogenic Substances <1 μg/m3
2019-00435401_H_EN respectively.
AgBB overview of results (3 days [µg/m³])
Name Value Unit
AgBB overview of results (28 days [µg/m³]) VOC without NIK <10000 μg/m3
Name Value Unit Carcinogenic Substances <10 μg/m3
TVOC (C6 ­ C16) <1000 μg/m3
Sum SVOC (C16 ­ C22) <100 μg/m3
8. References
Standards Category Rules for Construction Products from the
range of Environmental Product Declarations for
DIN EN 13501-1 Institut Bauen und Umwelt (IBU), Part B: Requirements
Klassifizierung von Bauprodukten und Bauarten zu on the EPD for Reaction resin products, 2019­01
ihrem Brandverhalten
DIN EN 14293
Klebstoffe ­ Klebstoffe für das Kleben von Parkett auf Further References
einen Untergrund ­ Prüfverfahren und
Mindestanforderungen AFNOR, «FD P01-015» 2006
Qualité environnementale des produits de construction
DIN EN ISO 50001 ­ Fascicule de données énergie et transport
DIN EN ISO 50001: 2018 Energy management
systems ­ Requirements with guidance for use AgBB (2018)
Vorgehensweise bei der gesundheitlichen Bewertung
EN 15804 der Emissionen von flüchtigen organischen
EN 15804:2012+A1:2013, Sustainability of Verbindungen (VVOC, VOC und SVOC) aus
construction works — Environmental Product Bauprodukten (2018)
Declarations — Core rules for the product category of
construction products. Candidate List of substances of very high concern
for Authorisation
EN 15804 European Cheminals Agency (ECHA), in accordance
EN 15804:2012+A2:2019, Sustainability of with Article 50(10) of the REACH regulation
construction works — Environmental Product
Declarations — Core rules for the product category of CDPH/EHLB/Standard Method V1.2
construction products. California CDPH Standard Method is a US standard for
evaluating and restricting VOC emissions to indoor air.
EN ISO 1183-1 Developed in California as "Section 01350"
DIN 51757:2011­01 Plastics ­ Methods for determining Specification, several systems in the US refer to CDPH
the density of non­cellular plastics ­ Part 1: Immersion Standard Method
method, liquid pyknometer method and titration
method Comité National Routier (CNR)
Enquête longue distance, PARIS, 2019
EN ISO 604
DIN EN ISO 604:2003­12: Determination of DIBt (2010)
compressive properties Grundsätze zur gesundheitlichen Bewertung von
Bauprodukten in Innenräumen (Oktober 2010)
ISO 14001 Eurofins test report, No. 392­2019­00435401_D_EN
ISO 14001:2015 Environmental management systems VOC test report for verification of compliance with
­ Requirements with guidance for use DIBt(2010)/AgBB(2018)
ISO 14025 Eurofins test report, No. 392-2019-00435401_E_EN
EN ISO 14025:2011, Environmental labels and VOC test report for verification of compliance with the
declarations — Type III environmental declarations — French VOC directive from 2019
Principles and procedures.
Eurofins test report, No. 392-2019-00435401_H_EN
PCR Part A VOC test report for verification of compliance with
Institut Bauen und Umwelt e.V, Berlin (pub.): Product CDPH/EHLB/Standard Method V1.2 (2017)
Category Rules for Construction Products from the
range of Environmental Product Declarations for European Waste code
Institut Bauen und Umwelt (IBU), Part A: Calculation in accordance with the European Waste Catalogue
Rules for the Life Cycle Assessment and (EWC) (EWC 2014/955/EU) Commission Decision
Requirements on the Project Report according to EN amending Decision 2000/532/EC on the list of waste
15804+A2:2019, 2021­04 pursuant to Directive 2008/98/EC of the European
Parliament and of the Council
PCR Part B
Institut Bauen und Umwelt e.V, Berlin (pub.): Product ETA 19/0665
10 Environmental Product Declaration Hilti AG – HIT­HY 200­R V3
European Technical Approval Hilti HIT­HY 200­R V3
Umwelt Bundesamt 2021
ETA 19/0600 Umwelt Bundesamt: Herkunftsnachweisregister
European Technical Approval Hilti HIT­HY 200­R V3 (HKNR) — Entwertungsnachweis durch GETECH
ENERGIE GMBH für HILTI
ETA 19/0601
European Technical Approval Hilti HIT­HY 200­R V3
ETA 20/0318 Database
European Technical Approval Hilti HIT­HY 200­R V3
Ecoinvent 3.8
ETA-19/0632 ecoinvent Version 3
European Technical Approval Hilti HIT­HY 200­R V3 Wernet, G., Bauer, C., Steubing, B., Reinhard, J.,
Moreno­Ruiz, E., and Weidema, B., 2016. The
French VOC Directives ecoinvent database version 3 (part I): overview and
Décret no 2011­321 du 23 mars 2011 relatif à methodology. The International Journal of Life Cycle
l’étiquetage des produits de construction ou de Assessment, [online] 21(9), pp.1218–1230. Available
revêtement de mur ou de sol et des peintures et vernis at: <http://link.springer.com/10.1007/s11367­016­1087­
sur leurs émissions de polluants volatils 8> [Accessed in 2021/2022].
Arrêté du 19 avril 2011 relatif à l’étiquetage des
produits de construction ou de revêtement de mur ou
de sol et des peintures et vernis sur leurs émissions de
polluants volatils Publication
ICC ESR-4878 IBU 2021
International code council (ICC), Evaluation report Institut Bauen und Umwelt e.V.: General Instructions
ESR­4878 HILTI HIT­HY 200 V3 (November 2021) for the EPD programme of Institut Bauen und Umwelt
e.V., Version 2.0, Berlin: Institut Bauen und Umwelt
ICC ESR-4868 e.V., 2021
International code council (ICC), Evaluation report www.ibu­epd.com
ESR­4868 HILTI HIT­HY 200 V3 (March 2022)
NSF
NSF/ANSI/CAN 61 Drinking Water System
Components ­ Health Effects
11 Environmental Product Declaration Hilti AG – HIT­HY 200­R V3
Publisher
Institut Bauen und Umwelt e.V. Tel +49 (0)30 3087748­ 0
Hegelplatz 1 Fax +49 (0)30 3087748­ 29
10117 Berlin Mail info@ibu­epd.com
Germany Web www.ibu-epd.com
Programme holder
Institut Bauen und Umwelt e.V. Tel +49 (0)30 ­ 3087748­ 0
Hegelplatz 1 Fax +49 (0)30 – 3087748 ­ 29
10117 Berlin Mail info@ibu­epd.com
Germany Web www.ibu-epd.com
Author of the Life Cycle
Assessment Tel +33 (0)9 53 23 98 30
ESTEANA Fax ­
Rue Mège 26 Mail contact@esteana.fr
83220 Le Pradet Web www.esteana.fr
France
Owner of the Declaration
Hilti Aktiengesellschaft Tel +423 234 2111
Feldkircher Strasse 100 Fax +423 234 2965
9494 Schaan Mail HAGHSE@hilti.com
Liechtenstein Web www.hilti.com
