ENVIRONMENTAL PRODUCT DECLARATION
as per ISO 14025 and EN 15804+A2
Owner of the Declaration dormakaba International Holding GmbH
Publisher Institut Bauen und Umwelt e.V. (IBU)
Programme holder Institut Bauen und Umwelt e.V. (IBU)
Declaration number EPD-DOR-20210012-CCA2-EN
Issue date 11.05.2021
Valid to 10.05.2026
Access manager 92 90 Wall
dormakaba
www.ibu-epd.com | https://epd-online.com
General Information
dormakaba Access manager 92 90 Wall
Programme holder Owner of the declaration
IBU – Institut Bauen und Umwelt e.V. dormakaba International Holding GmbH
Hegelplatz 1 DORMA Platz 1
10117 Berlin 58256 Ennepetal
Germany Germany
Declaration number Declared product / declared unit
EPD-DOR-20210012-CCA2-EN 1 piece of the product: Access manager 92 90 Wall
This declaration is based on the product category rules: Scope:
Electronic and physical Access Control Systems, 01.08.2021 This EPD refers to a specific product manufactured by dormakaba. The
(PCR checked and approved by the SVR) production site is located in Villingen-Schwenningen (Germany), and the
year of data collection is 2019.
The owner of the declaration shall be liable for the underlying information
Issue date and evidence; the IBU shall not be liable with respect to manufacturer
information, life cycle assessment data and evidences.
11.05.2021
The EPD was created according to the specifications of EN 15804+A2. In
the following, the standard will be simplified as EN 15804.
Valid to
10.05.2026 Verification
The standard EN 15804 serves as the core PCR
Independent verification of the declaration and data according to ISO
14025:2011
internally X externally
Dipl.-Ing. Hans Peters
(Chairman of Institut Bauen und Umwelt e.V.)
Florian Pronold Dr.-Ing. Wolfram Trinius,
(Managing Director Institut Bauen und Umwelt e.V.) (Independent verifier)
1 Environmental Product Declaration - dormakaba - Access manager 92 90 Wall
Product
Host Interface
Product description/Product definition • Ethernet 10/100 Mbit/s
The dormakaba access manager 92 90 as a central access
control manager meets all the requirements of modern access Peripherals Interface
control. Thanks to its intelligent decision logic and free • 2x RS-485/RS-422Inputs/outputs
parametrisation, it controls all access events, at basic access • 16 potential-free relays, 30 V AC/48 V DC; max. 1 A
points as well as to complex, highly sensitive company areas. • 18 galvanically isolated digital Inputs
Predefined configurations simplify the setting of individual door
functions. The state-of-the-art IT security is based on a modern Power supply
operating system and TLS (Transport Layer Security) Input voltage - 230 V AC 50 Hz max. 150 VA - 115V AC 60 Hz
encryption that can be activated between controller and host max. 150 VA - 24 V DC max. 100 W
system: the control electronics integrates all the necessary Output voltage - 2 x 24 V DC max. 40 W - 1 x 12 V AC max. 20
requirements to enable a connection to Cloud Services via IoT. VA
Therefore, the access manager 92 90 is already designed for Class of protection as per BS EN 60529: IP20
the requirements of tomorrow.
Switching to other dormakaba access solutions at a later point The product is not harmonised in accordance with the
is also possible. For the placing on the market in the European Construction Product Regulations (CPR) but in accordance with
Union/European Free Trade Association (EU/EFTA) (with the other provisions for harmonisation of the EU. Compliance with
exception of Switzerland) the following legal provisions apply: the European Union Directive and technical specifications:
• Electromagnetic Compatibility Directive (EMC) • EN 55032:2015
• Low Voltage Directive (LVD) • EN 55024:2016
• Restriction of Hazardous Substances (RoHS) • EN 61000-3-2:2014
• EN 50581:2012 • EN 61000-3-3:2013
The CE-marking takes into account the proof of conformity with • EN 62368-1:2014 + A11:2017
the respective harmonized standards based on the legal The product is subject to CE marking according to the relevant
provisions above. For the application and use the respective harmonization legislation.
national provisions apply. In addition, the product also conforms to the following
standards:
Application
• UL 294:2013
Central Access control
• UL 62368-1:2014
An access manager is installed in a protected environment and
• CAN/CSA-22.2 No. 62368-1:2014
uses various test criteria to check whether a booking made on a
reader is authorized or not.
Base materials/Ancillary materials
The major material compositions of the product are listed
Door management
below:
• Personnel interlock control
• Door activation Name Value Unit
• Monitoring of door opening Stainless Steel 0.2 %
• Monitoring of door opening time Steel 72.4 %
• Access monitoring
Plastics 0.6 %
Cable 2.4 %
Alarm Management
Electronics 24.3 %
The access manager reports irregularities in access control or
door management to the host computer. An additional function Paper <0.1 %
is to activate relays. Other Metals 0.1 %
Technical Data The product includes partial articles which contain substances
listed in the Candidate List of REACH
The access manager 92 90 Wall has the following technical
properties:
Regulation 1907/2006/EC (date: 08.07.2021) exceeding 0.1
Name Value Unit
percentage by mass in the alloy: yes
Operating Temperature 0 - 40 °C
• Lead titanium trioxide (O3PbTi): 12060-00-03
Operating Humidity 5 - 85 %
The Candidate List can be found on the ECHA website
Width Dimension 300 mm
address: https:echa.europa.eu/de/home.
Height Dimension 410 mm
Reference service life
Depth Dimension 120 mm
The reference service life of the dormakaba access manager
Weight 9,46 kg
92 90 Wall is estimated to be 15 years. This number is based
Power consumption "on mode" 12 W
on the support and service life and is not an estimated lifetime.
Power consumption "idle mode" 5 W
LCA: Calculation rules
Declared unit
Declared Unit
The declared unit is 1 piece of the product: Access manager 92
90 Wall.
2 Environmental Product Declaration - dormakaba - Access manager 92 90 Wall
Name Value Unit
End-of-life stage– Modules C1-C4 and D
Declared unit 1 pce.
The end-of-life stage includes:
Conversion factor to 1 kg (kg per declared unit) 11.676 -
— C1, de-construction, demolition:
— C2, transport to waste processing; — C3, waste processing
System boundary
for reuse, recovery and/or recycling;
The type of EPD is: cradle to gate with options, modules C1– — C4, disposal;
C4, and module D (A1–A3 + C + D and additional modules: A4
+ A5 + B6) Production - Module A1-A3 including provision and all transport, provision of all materials,
The product stage includes: products and related energy and water use.
— A1, raw material extraction, processing and mechanical
treatments, processing of secondary material input (e.g. Module D (Benefits and loads beyond the system boundary)
recycling processes), — A2, transport to the manufacturer, — includes:
A3, manufacturing and assembly including provision of all — D, recycling potentials, expressed as net impacts and
materials, products and energy, as well as waste processing up benefits.
to the end-of waste state.
Geographic Representativeness
Construction stage - Modules A4-A5 Land or region, in which the declared product system is
The construction process stage includes: manufactured, used or handled at the end of the product´s
— A4, transport to the building site; — A5, installation into the lifespan: Germany
building; including provision of all materials, products and
energy, as well as waste processing up to the end-of-waste
state or disposal of final residues during the construction Comparability
process stage. Basically, a comparison or an evaluation of EPD data is only
possible if all the data sets to be compared were created
Use stage - Module B6 according to EN 15804 and the building context, respectively
The use stage related to the operation of the building includes: the product-specific characteristics of performance, are taken
— B6, operational energy use into account. Background database: GaBi, SP40.
LCA: Scenarios and additional technical information
Name Value Unit
Characteristic product properties of biogenic carbon
Life Span according to the manufacturer 15 a
Information on describing the biogenic Carbon Content at
factory gate Operational energy use (B6) and Operational water use
(B7)
Name Value Unit
The use stage is declared for 15 years.
kg
Biogenic carbon content in product 0.00051
C Name Value Unit
Biogenic carbon content in accompanying kg Energy consumption for 1 year 54.02 kWh
0.946
packaging C on mode per day 4 h
Note: 1 kg of biogenic carbon is equivalent to 44/12 kg of CO . idle mode 20 h
2
on mode power 12 W
idle mode 5 W
The following technical scenario information is required for the Days per year in use 365 days
declared modules.
End of life (C1-C4)
Transport to the building site (A4)
C1: The product dismantling from the building is done manually
Name Value Unit
without environmental burden.
Litres of fuel 0.032 l/100km
Name Value Unit
Transport distance 100 km
Recycling (Plastic) 7.308 kg
Capacity utilisation (including empty runs) 51 %
Energy recovery (Plastic) 0.311 kg
Transport distance is declared for a distance of 100km by truck
Landfilling 1.837 kg
in order to allow scaling to a specific point of installation.
Transportation to Waste Processing Site 50 km
Region for end of life: Global
Installation into the building (A5)
Name Value Unit
Reuse, recovery and/or recycling potentials (D), relevant
Waste Packaging (paper) 2.2 kg scenario information
Waste Packaging (plastic) 0.02 kg Collection rate is 100%.
Reference service life
3 Environmental Product Declaration - dormakaba - Access manager 92 90 Wall
LCA: Results
Disclaimer EP-freshwater: This indicator has been calculated as 'kg P eq' as required in the characterization model (EUTREND
model, Struijs et al., 2009b, as implemented in ReCiPe; http://eplca.jrc.ec.europa.eu/LCDN/developerEF.xhtml).
DESCRIPTION OF THE SYSTEM BOUNDARY (X = INCLUDED IN LCA; MND = MODULE OR INDICATOR NOT DECLARED; MNR
= MODULE NOT RELEVANT)
Benefits and
Construction loads beyond
Product stage Use stage End of life stage
process stage the system
boundaries
la ire ta m w a Ry lp p u s tro p s n a rT g n iru tc a fu n a M e h t m o rf tro p s n a rTe tis e h t o t e ta g y lb m e s s A e s U e c n a n e tn ia M ria p e R tn e m e c a lp e R tn e m h s ib ru fe R y g re n e la n o ita re p Oe s u re ta w la n o ita re p Oe s u n o itc u rts n o c -e Dn o itilo m e d tro p s n a rT g n is s e c o rp e ts a W la s o p s iD -e s u e R-y re v o c e R-g n ilc y c e Rla itn e to p
A1 A2 A3 A4 A5 B1 B2 B3 B4 B5 B6 B7 C1 C2 C3 C4 D
X X X X X MND MND MNR MNR MNR X MND X X X X X
RESULTS OF THE LCA - ENVIRONMENTAL IMPACT according to EN 15804+A2: 1 piece Access manager 92 90 Wall
Parameter Unit A1-A3 A4 A5 B6 C1 C2 C3 C4 D
GWP-total kg CO 2 eq 4.76E+01 1.02E-01 3.17E+00 3.28E+02 0 3.83E-02 1.44E-01 2.8E-02 -2.31E+00
GWP-fossil kg CO 2 eq 5.02E+01 9.76E-02 1.29E-01 3.26E+02 0 3.66E-02 1.44E-01 2.79E-02 -2.31E+00
GWP-biogenic kg CO 2 eq -2.72E+00 4.51E-03 3.04E+00 1.09E+00 0 1.69E-03 3.35E-06 9.52E-05 1.26E-03
GWP-luluc kg CO 2 eq 7E-02 2.32E-06 5.42E-05 4.73E-01 0 8.72E-07 8.13E-06 8.02E-05 -3.17E-03
ODP kg CFC11 eq 3.49E-09 1.03E-17 5.88E-16 7.18E-12 0 3.87E-18 7.26E-17 1.03E-16 -1.71E-14
AP mol H+ eq 3E-01 9.77E-05 8.83E-04 7.2E-01 0 3.67E-05 2.56E-05 2E-04 -2.54E-02
EP-freshwater kg P eq 3.38E-04 2.09E-08 1.14E-07 8.71E-04 0 7.84E-09 1.16E-08 4.78E-08 -2.34E-06
EP-marine kg N eq 4.55E-02 3.11E-05 3.17E-04 1.6E-01 0 1.17E-05 5.78E-06 5.14E-05 -2.06E-03
EP-terrestrial mol N eq 4.82E-01 3.46E-04 3.97E-03 1.68E+00 0 1.3E-04 1.17E-04 5.65E-04 -2.22E-02
kg NMVOC
POCP 1.37E-01 8.79E-05 8.42E-04 4.38E-01 0 3.3E-05 1.6E-05 1.56E-04 -6.72E-03
eq
ADPE kg Sb eq 1.06E-02 2.93E-09 9.23E-09 9.44E-05 0 1.1E-09 9.95E-10 2.5E-09 -1.13E-03
ADPF MJ 6.11E+02 1.38E+00 1.01E+00 5.73E+03 0 5.2E-01 6.67E-02 3.66E-01 -3.37E+01
m3 world eq
WDP 1.35E+01 1.91E-04 3.92E-01 7.11E+01 0 7.18E-05 1.47E-02 2.92E-03 -7.74E-01
deprived
GWP = Global warming potential; ODP = Depletion potential of the stratospheric ozone layer; AP = Acidification potential of land and water; EP =
Eutrophication potential; POCP = Formation potential of tropospheric ozone photochemical oxidants; ADPE = Abiotic depletion potential for non-fossil
resources; ADPF = Abiotic depletion potential for fossil resources; WDP = Water (user) deprivation potential)
RESULTS OF THE LCA - INDICATORS TO DESCRIBE RESOURCE USE according to EN 15804+A2: 1 piece Access manager 92
90 Wall
Parameter Unit A1-A3 A4 A5 B6 C1 C2 C3 C4 D
PERE MJ 1.56E+02 4.36E-03 2.66E+01 2.54E+03 0 1.64E-03 3.16E-02 4.79E-02 -6.31E+00
PERM MJ 2.64E+01 0 -2.64E+01 0 0 0 -1.43E-02 0 0
PERT MJ 1.83E+02 4.36E-03 1.85E-01 2.54E+03 0 1.64E-03 1.73E-02 4.79E-02 -6.31E+00
PENRE MJ 6.04E+02 1.39E+00 1.87E+00 5.74E+03 0 5.2E-01 6.45E+00 3.66E-01 -3.37E+01
PENRM MJ 7.24E+00 0 -8.6E-01 0 0 0 -6.38E+00 0 0
PENRT MJ 6.12E+02 1.39E+00 1.01E+00 5.74E+03 0 5.2E-01 6.67E-02 3.66E-01 -3.37E+01
SM kg 7.49E+00 0 0 0 0 0 0 0 0
RSF MJ 0 0 0 0 0 0 0 0 0
NRSF MJ 0 0 0 0 0 0 0 0 0
FW m3 3.29E-01 7.83E-06 9.23E-03 2.94E+00 0 2.94E-06 3.52E-04 9.22E-05 -1.65E-02
PERE = Use of renewable primary energy excluding renewable primary energy resources used as raw materials; PERM = Use of renewable primary
energy resources used as raw materials; PERT = Total use of renewable primary energy resources; PENRE = Use of non-renewable primary energy
excluding non-renewable primary energy resources used as raw materials; PENRM = Use of non-renewable primary energy resources used as raw
materials; PENRT = Total use of non-renewable primary energy resources; SM = Use of secondary material; RSF = Use of renewable secondary fuels;
NRSF = Use of non-renewable secondary fuels; FW = Use of net fresh water
RESULTS OF THE LCA – WASTE CATEGORIES AND OUTPUT FLOWS according to EN 15804+A2:
1 piece Access manager 92 90 Wall
Parameter Unit A1-A3 A4 A5 B6 C1 C2 C3 C4 D
HWD kg 2.87E-05 1.34E-10 1.54E-09 2.37E-06 0 5.04E-11 2.54E-10 5.57E-09 1.06E-07
NHWD kg 3.11E+00 1.42E-04 1.03E-01 4.07E+00 0 5.32E-05 1.49E-02 1.84E+00 -3.36E-01
RWD kg 1.71E-02 1.49E-06 5.26E-05 8.7E-01 0 5.58E-07 2.48E-06 4.16E-06 -1.51E-03
CRU kg 0 0 0 0 0 0 0 0 0
MFR kg 0 0 0 0 0 0 7.38E+00 0 0
MER kg 0 0 0 0 0 0 0 0 0
EEE MJ 8.58E-01 0 4.81E+00 0 0 0 0 0 0
4 Environmental Product Declaration - dormakaba - Access manager 92 90 Wall
EET MJ 1.56E+00 0 8.77E+00 0 0 0 0 0 0
HWD = Hazardous waste disposed; NHWD = Non-hazardous waste disposed; RWD = Radioactive waste disposed; CRU = Components for re-use;
MFR = Materials for recycling; MER = Materials for energy recovery; EEE = Exported electrical energy; EET = Exported thermal energy
RESULTS OF THE LCA – additional impact categories according to EN 15804+A2-optional:
1 piece Access manager 92 90 Wall
Parameter Unit A1-A3 A4 A5 B6 C1 C2 C3 C4 D
Disease
PM 3.07E-06 5.14E-10 4.95E-09 6.04E-06 0 1.93E-10 3.27E-10 2.47E-09 -2.05E-07
incidence
IR kBq U235 eq 1.69E+00 2.13E-04 8.09E-03 1.43E+02 0 7.98E-05 2.23E-04 4.28E-04 -2.44E-01
ETP-fw CTUe 2.96E+02 9.81E-01 4.76E-01 2.45E+03 0 3.68E-01 2.5E-02 2.09E-01 -1.49E+01
HTP-c CTUh 4.17E-08 1.85E-11 2.55E-11 6.78E-08 0 6.93E-12 2.17E-12 3.09E-11 -1.07E-09
HTP-nc CTUh 1.08E-06 7.89E-10 1.15E-09 2.5E-06 0 2.96E-10 2.19E-10 3.41E-09 -7.13E-08
SQP SQP 5.44E+02 3.56E-03 2.68E-01 1.83E+03 0 1.34E-03 2E-02 7.62E-02 -1.34E+01
PM = Potential incidence of disease due to PM emissions; IR = Potential Human exposure efficiency relative to U235; ETP-fw = Potential comparative
Toxic Unit for ecosystems; HTP-c = Potential comparative Toxic Unit for humans (cancerogenic); HTP-nc = Potential comparative Toxic Unit for humans
(not cancerogenic); SQP = Potential soil quality index
Disclaimer 1 – for the indicator IRP This impact category deals mainly with the eventual impact of low dose ionizing radiation on human
health of the nuclear fuel cycle. It does not consider effects due to possible nuclear accidents, occupational exposure nor due to
radioactive waste disposal in underground facilities. Potential ionizing radiation from the soil, from radon and from some construction
materials is also not measured by this indicator.
Disclaimer 2 – for the indicators ADPE, ADPF, WDP, ETP-fw, HTP-c, HTP-nc, SQP The results of this environmental impact indicator
shall be used with care as the uncertainties on these results are high or as there is limited experience with the indicator.
References
Standards Electromagnetic Compatibility Directive
Directive 2014/30/EU of the European Parliamant and of the
CAN/CSA-22.2 No. 62368-1:2014 Council of 26 February 2014 on the harmonisation of the laws
Audio/video, information and communication of the Member States relating to electromagnetic compatibility.
technologyequipment — Part 1: Safety requirements.
ISO 14025:2011-10
EN 15804:2019+A2 DIN EN ISO 14025:2011-10, Environmental labels and
EN 15804:2019+A2 (in press), Sustainability of construction declarations — Type III environmental declarations —
works — Environmental Product Declarations — Core rules for Principles and procedures.
the product category of construction products.
Low Voltage Directive (LVD)
EN 50581:2012 Directive 2014/35/EU of the European Parliament and of the
Technical documentation for the assessment of electrical and Council of 26 February 2014 on the harmonisation of the laws
electronic products with respect to the restriction of hazardous of the Member States relating to the making available on the
substances. market of electrical equipment designed for use within certain
voltage limits.
EN 55024:2016
Information technology equipment - Immunity characteristics - Radio Equipment Directive (RED)
Limits and methods of measurement. Directive 2014/53/EU of the European Parliament and of the
Council of 16 April 2014 on the harmonisation of the laws of the
EN 55032:2015 Member States relating to the making available on the market
Electromagnetic compatibility of multimedia equipment - of radio equipment and repealing Directive 1999/5/EC.
Emission Requirements.
Registration, Evaluation, Authorisation and Restriction of
EN 60529:2014 Chemicals (REACH)
Degrees of protection provided by enclosures (IP 20). Regulation (EC) No 1907/2006 of the European Parliament and
of the Council on the Registration, Evaluation, Authorisation
EN 61000-3-2:2013 and Restriction of Chemicals (REACH).
Electromagnetic compatibility (EMC) - Part 3-2: Limits - Limits
for harmonic current emissions (equipment input current ≤ 16 A Restriction of Hazardous Substances (RoHS)
per phase). Directive on the restriction of the use of certain hazardous
substances in electrical and electronic equipment (RoHS),
EN 61000-3-3:2013 Directive (EU) No 2011/65.
Electromagnetic compatibility (EMC) - Part 3-3: Limits -
Limitation of voltage changes, voltage fluctuations and flicker in UL 294:2013
public low-voltage supply systems, for equipment with rated UL Standard for Safety Access Control System Unit.
current ≤ 16 A per phase and not subject to conditional
connection. UL 62368-1:2014
Standard for Audio/video, information and communication
EN 62368-1:2014+A11:2017 technology equipment - Part 1: Safety requirements.
Audio/video, information and communication technology
equipment - Part 1: Safety requirements. Further References
5 Environmental Product Declaration - dormakaba - Access manager 92 90 Wall
IBU 2016 LCA-tool dormakaba
Institut Bauen und Umwelt e.V.: General Programme LCA tool, version 1.0.
Instructions for the Preparation of EPDs at the Institut Bauen Developed by Sphera Solutions GmbH.
und Umwelt e.V. Version 1., Berlin: Institut Bauen und Umwelt
e.V., 2016. www.ibu-epd.com GaBi ts software PCR Part A
Sphera Solutions GmbH PCR – Part A:
Gabi Software System and Database for Life Cycle Engineering Calculation Rules for the Life Cycle As-sessment and
1992-2020 Version 10.0.0.71 University of Stuttgart Leinfelden- Requirements on the Project Re-port according to EN
Echterdingen 15804+A2:2019, Version 1.0, Institut Bauen und Umwelt e.V.,
www.ibu-epd.com.
GaBi ts documentation
GaBi life cycle inventory data documentation (https://www.gabi- PCR Part B
software.com/support/gabi/gabi-database-2020-lci- PCR – Part B: Requirements on the EPD for Building Hardware
documentation/). product, version 1.2, Institut Bauen und Umwelt e.V., www.ibu-
epd.com, 2017.
6 Environmental Product Declaration - dormakaba - Access manager 92 90 Wall
Publisher
Institut Bauen und Umwelt e.V. +49 (0)30 3087748- 0
Hegelplatz 1 info@ibu-epd.com
10117 Berlin www.ibu-epd.com
Germany
Programme holder
Institut Bauen und Umwelt e.V. +49 (0)30 3087748- 0
Hegelplatz 1 info@ibu-epd.com
10117 Berlin www.ibu-epd.com
Germany
Author of the Life Cycle Assessment
Sphera Solutions GmbH +49 711 341817-0
Hauptstraße 111- 113 info@sphera.com
70771 Leinfelden-Echterdingen www.sphera.com
Germany
Owner of the Declaration
dormakaba International Holding GmbH +49 2333 793-0
DORMA Platz 1 info.de@dormakaba.com
58256 Ennepetal www.dormakaba.com
Germany
7 Environmental Product Declaration - dormakaba - Access manager 92 90 Wall
