ENVIRONMENTAL PRODUCT DECLARATION
as per ISO 14025 and EN 15804+A2
Owner of the Declaration Hilti Aktiengesellschaft
Publisher Institut Bauen und Umwelt e.V. (IBU)
Programme holder Institut Bauen und Umwelt e.V. (IBU)
Declaration number EPD-HIL-20240323-IBA1-EN
Issue date 05/06/2024
Valid to 04/06/2029
Aluminium profiles
Hilti Aktiengesellschaft
www.ibu-epd.com | https://epd-online.com
1. General Information
Hilti Aktiengesellschaft Aluminium profiles
Programme holder Owner of the declaration
IBU – Institut Bauen und Umwelt e.V. Hilti Aktiengesellschaft
Hegelplatz 1 Feldkircher Strasse 100
10117 Berlin 9494 Schaan
Germany Liechtenstein
Declaration number Declared product / declared unit
EPD-HIL-20240323-IBA1-EN The declared product is 1 kg of aluminium profiles.
This declaration is based on the product category rules: Scope:
Products of aluminium and aluminium alloys, 01/08/2021 This product declaration refers to a declared unit of 1 kg of aluminium
(PCR checked and approved by the SVR) profiles produced in one production facility in Romania. The owner of the
declaration shall be liable for the underlying information and evidence; the
IBU shall not be liable with respect to manufacturer information, life cycle
Issue date assessment data and evidences.
The owner of the declaration shall be liable for the underlying information
05/06/2024
and evidence; the IBU shall not be liable with respect to manufacturer
information, life cycle assessment data and evidences.
Valid to
The EPD was created according to the specifications of EN 15804+A2. In
04/06/2029 the following, the standard will be simplified as EN 15804.
Verification
The standard EN 15804 serves as the core PCR
Independent verification of the declaration and data according to ISO
14025:2011
internally X externally
Dipl.-Ing. Hans Peters
(Chairman of Institut Bauen und Umwelt e.V.)
Florian Pronold Dr. Eva Schmincke,
(Managing Director Institut Bauen und Umwelt e.V.) (Independent verifier)
1 Environmental Product Declaration - Hilti Aktiengesellschaft - Aluminium profiles
2. Product
2.1 Product description/Product definition No biocidal products have been added to the present
This EPD refers to 1 kilogram of aluminium profiles, construction product or it has been treated with biocidal
represented by profiles of different shapes coming from the products (it is thus a treated product within the meaning of the
extrusion process. The final products are identical in terms of Biocidal Products Regulation (EU) No 528/2012).
chemical composition and production process; the only
difference between the products is the shape. The aluminium 2.6 Manufacture
profiles are uncoated and non-insulated. The main technological flow is the extrusion of aluminium bars
For the use and application of the product, the respective and transforming them into uncoated aluminium profiles. The
national provisions at the place of use apply. extrusion activity is carried out in several stages, as follows:
2.2 Application
The final aluminium product (aluminium profiles) is used for
creating different aluminium products for the Building &
construction sector.
2.3 Technical Data
The final product has the technical characteristics described in
the table below
Constructional data
Name Value Unit
Gross density 2.7 kg/m3
Melting point 655 °C
Electrical conductivity at 20°C 34 m/Ωmm2
Thermal conductivity 220 W/(mK)
Coefficient of thermal expansion 23.4 10-6K-1
Modulus of elasticity 69.5 N/mm2
Shear modulus 26.1 N/mm2
Specific heat capacity 898 kJ/kgK
There are several production lines with interchangeable moulds
Hardness 90 HB
which will define the aluminium profile shape. The aluminium
Yield strength Rp 0,2 min. 225 N/mm2
billets are fed to the extrusion equipment with a conveyor,
Tensile strength Rm min. 270 N/mm2 heated to a temperature at which Aluminium becomes easier to
Tensile stress at break 25 % be formed and then extruded into the final shape. The profiles
are then transferred to a curing oven which uses natural gas to
Note that for the Electrical conductivity at 20 °C, Thermal
heat the aluminium profiles and where the profiles are kept in
conductivity, Hardness, Yield strength Rp 0,2 min., Tensile
order to be cured. The industrial products made are intended
strength Rm min. and Tensile stress at break, the values
for the Business-to-business market segment.
represent the maximum values.
These stages use mainly electricity and natural gas, as well as
a small quantity of chemicals and industrial gases. Diesel is
Performance data of the product with respect to its
consumed for internal transport activities. The sodium
characteristics in accordance with the relevant technical
hydroxide solution is used in the moulds cleaning process,
provision (no CE-marking).
through which residual aluminium is removed from the moulds.
The company has implemented a certified quality management
2.4 Delivery status
system, ISO 9001, which monitors the entire manufacturing
The aluminium profiles are delivered on the desired length and
process.
shape. The profiles are secured during transport by being tied
together using plastic bands and placed on rectangular wooden
bars.
2.5 Base materials/Ancillary materials
2.7 Environment and health during manufacturing
The main constituent of the aluminium profiles, is aluminium.
The production facility has an environmental management
The share of virgin and recycled aluminium in the billets
system in accordance with ISO 14001 and an occupational
depend on the recipe of different manufacturers. Based on the
health and safety management system in accordance with ISO
information provided by the suppliers of billets, around 60 % of
45001 in order to ensure environmental protection and
the aluminium in the profiles is primary aluminium and 40 % of
occupational health and safety in the production process.
the aluminium is recycled.
The product does not contain substances on the ECHA list of 2.8 Product processing/Installation
Substances of Very High Concern (SVHC) above 0.1 mass %.
The final aluminium product (aluminium profiles) is used for
creating different aluminium products for: the building &
construction sector.
The product does not contain other carcinogenic, mutagenic,
reprotoxic (CMR) substances of category 1A or 1B not on the 2.9 Packaging
candidate list above 0.1 mass % in at least one sub-product. The profiles are tied together using plastic straps, at a length
based on clients' specifications, packed in cardboard for being
2 Environmental Product Declaration - Hilti Aktiengesellschaft - Aluminium profiles
secured during transportation and placed on wooden bars. The toxicity of fire gases is not applicable.
The wooden bars, the plastic straps and the cardboard can be
Fire protection
recycled by the customer.
Name Value
2.10 Condition of use Building material class A1
There are no special features of the material composition for Burning droplets not applicable
the period of use.
Smoke gas development not applicable
2.11 Environment and health during use
If the aluminium profiles are used as intended, no hazards to Water
air, water and soil as well as to human health can arise. The exposure of the aluminium profiles to water does not alter
the product and has no negative impact on the environment
No harmful substances are incorporated in the product. (water).
The environmental impact during the use phase depends on Mechanical destruction
the design of the end product since aluminium profiles are not Unforeseen mechanical destruction of the aluminium profiles is
final products. not relevant.
2.12 Reference service life 2.14 Re-use phase
The aluminium profiles are not a final product and they are The aluminium profiles are 100 % recyclable. The material does
used for different industries as input material where it can have not suffer any loss of quality and can be recycled forever. The
multiple applications, therefore no reference service life (RSL) aluminium scrap from demolition can be separated, collected
is declared for aluminium profiles. and recycled by the recycling industry.
2.15 Disposal
Each industry might treat the aluminium profiles based on the
properties of the environment where the finished products will According to the European Waste Catalog (EWC), the disposal
stand. The treatment will influence the ageing of the final code depends on the end product.
product. Given its high value, the aluminium scrap it's not disposed but
used as a raw material in the recycling industry.
2.13 Extraordinary effects
2.16 Further information
Fire
Aluminium profiles meet the requirements of building material For more information, visit: https://www.hilti.com/
class A "non-combustible" according to DIN 4102-4. The
melting point of aluminium is approx. 650° C.
3. LCA: Calculation rules
• The transport of the raw and ancillary materials was
3.1 Declared Unit calculated based on the actual distances of the
The declared unit refers to 1 kilogram of aluminium profiles, suppliers.
represented by profiles of different shapes coming from the • The energy consists of diesel used in the manufacturing
extrusion process. Final products are identical in terms of process and natural gas which is supplied from the
chemical composition and production process; the only national grid.
difference between the products is the shape. Products • The electricity is 100 % green electricity based on the
manufacturing is located at one plant in Romania refers to the contract concluded between the production facilitiy and
same technology. The product consists of aluminium profiles the electricity supplier.
using raw materials (aluminium billets) from several suppliers. Module C2 | Transport to waste processing
The share of virgin aluminium in the aluminium bars is assumed Module C2 declares the environmental impacts resulting from
to be 60 % while the rest of 40 % is assumed to be recycled transporting the waste aluminium to a waste processing facility
aluminium, as reported by the suppliers. at an assumed distance of 50 km.
Data used in calculations represent site-specific production
volumes for 2022 of the main product line. There are no by-
products formed from the production line subject to this study. Module C3 | Waste processing
Module C3 declares the environmental impacts resulting from
Declared unit and mass reference the treatment of aluminium scrap by collecting, sorting, cleaning
and pressing (90 % of the product).
Name Value Unit
Declared unit 1 kg
Module C4 | Disposal
3.2 System boundary Module C4 declares the environmental impacts resulting from
The LCA for aluminium profiles is a cradle-to-gate assessment landfilling (10 % of the product).
of the environmental impacts with options. Module D | Credits and loads outside the system boundary
The following life cycle phases are considered in the analysis: In Module D, the net substitution potential of primary aluminium
through a recycling scenario (90 % of the product) is presented.
Module A1-A3 | Product stage
The following processes were considered: 3.3 Estimates and assumptions
This study analysis is based mainly on-site specific data related
• The purchase of the raw materials and the ancillary
to products manufacturing. Study results are valid for the
materials such as primary aluminium, recycled
technological process specified, geographical area and time
aluminium as well as ancillary materials such as alloying
period mentioned.
metals and packaging.
3 Environmental Product Declaration - Hilti Aktiengesellschaft - Aluminium profiles
Furthermore, the following estimates have been made: be not more than 1 % of renewable and non-renewable primary
energy usage and not more than 1 % of the total mass flow for
• PP and PET were assumed to be used in a share of 25
a single flow and 99 % of all flows should be considered.
% PP and 75 % PET from the total amount of plastic
packaging materials.
3.5 Background data
• It was assumed that soft sawnwood with a density of
Calculations were performed using Simapro 9.5, where inputs
540 kg/m3 is used for wood packaging.
and outputs are listed. The LCA impacts were calculated using
• waste outputs such as mixed plastic, wood, and
characterization factors from Ecoinvent 3.9.1 database,
cardboard, are accounted for by selecting data sets
applying the EN 15804 + A2 Method V1.03/EF 3.1
representative for the market, where transport is already
normalization and weighting set.
included in the final assessment of the impacts.
• It is assumed that the water needed for the sodium 3.6 Data quality
hydroxide solution was the difference between the Data reliability is ensured by the manufacturer's data
sodium hydroxide as an input and the waste solution. management systems and expert knowledge of plant
Water use is declared as water from a well. In the engineers. Additional questions regarding reported values (e.g.,
calculations, the total amount of water is classified as type of material, materials use, waste management techniques,
tap water - underground water without treatment since transportation distances, etc.) were answered and clarified by
characterisation factors in Ecoinvent 3.9.1 suitable for plant engineers.
water from a well are not available.
• Aluminium bars produced from the main supplier are 3.7 Period under review
accounted for in the modelling process with product- Site-specific data is collected for all flows according to the set
specific environmental burden, while for the aluminium cut-off criteria. Data collected is representative of the same
sourced from other suppliers a 20 %, 60 % and 100 % technology for the period between the 1st of January 2022 to
virgin material is assumed, depending on the supplier. the 31st of December 2022. All collected data is based on the
• Starting with 2021, the production facility purchases only
actual quantities used and produced during this period.
green electricity. The electricity mix of 62.41 % hydro-
power and 37.59 % wind power used in this study is for 3.8 Geographic Representativeness
the year 2021. The share of renewable electricity for the Land or region, in which the declared product system is
year 2022 will be published by the electricity supplier manufactured, used or handled at the end of the product´s
after the completion of this study. lifespan: Europe
• The input of PVC was excluded, as this life cycle
assessment study is performed for uncoated aluminium
profiles and the total production was assumed to be 3.9 Allocation
without PVC. In this study, there are no by-products and thus no relevant
• For wood, the only available input was in pieces. It was allocation is considered necessary since all inputs are
assumed a 10x10x10 cm cube, 0.0001 m3 per piece. converted to the main product described above and waste
• For cardboard, the only available input was in pieces. A outflows.
weight of 0.01 kg/ piece was assumed. The total environmental burden is associated with the products
Assumptions applied for transport are summarized below: delivered to the customers.
• the use of Euro 5 and 6 trucks is assumed for the 3.10 Comparability
transport of aluminium bars, due to the prevalence of
Basically, a comparison or an evaluation of EPD data is only
this type of Euro trucks in the fleet transporting
possible if all the data sets to be compared were created
materials.
according to EN 15804 and the building context, respectively
• all inputs, except aluminium bars retreived from the
the product-specific characteristics of performance, are taken
main supplier, sodium hydroxide, are accounted for by
into account. Calculations were performed using Simapro 9.5,
selecting data sets representative for the market, where
where inputs and outputs are listed. The LCA impacts were
transport is already included in the final assessment of
calculated using characterization factors from Ecoinvent 3.9.1
the impacts.
database. No biogenic carbon is contained in the declared
• The average distance for the packaging waste, was
product.
assumed 250 km.
End of life (C1-C4)
For the end-of-life scenario used in this study the following
3.4 Cut-off criteria
assumptions are made: 90 % of the aluminium is recycled and
All inputs and outputs from background system to foreground
10 % of the aluminium is landfilled at the end of life and thus
system processes, with significant potential impact, are
follows the most recent data on aluminium recycling published
included in the calculation. Company specific-data is
by the European Aluminium Association.
available for all foreground processes. Cut-off criteria are set to
4. LCA: Scenarios and additional technical information
Name Value Unit
Characteristic product properties of biogenic carbon
kg
Biogenic carbon is present only in the wooden packaging. Biogenic carbon content in product -
C
Information on describing the biogenic carbon content at Biogenic carbon content in accompanying 8.39E- kg
factury gate packaging 09 C
The biogenic carbon was calculated only from the sum of
Note: 1 kg of biogenic carbon is equivalent to 44/12 kg of CO .
packaging. 2
4 Environmental Product Declaration - Hilti Aktiengesellschaft - Aluminium profiles
End of life (C1-C4) Reuse, recovery and/or recycling potentials (D), relevant
For the end-of-life scenario used in this study the following scenario information
assumptions are made: 90 % of the aluminium is recycled and Name Value Unit
10 % of the aluminium is landfilled at the end of life and thus
Recycling 90 %
follows the most recent data on aluminium recycling published
by the European Aluminium Association.
Name Value Unit
Recycling 0.9 kg
Landfilling 0.1 kg
5 Environmental Product Declaration - Hilti Aktiengesellschaft - Aluminium profiles
5. LCA: Results
The following table shows the LCA results for the declared unit of 1 kg of aluminium profiles.
DESCRIPTION OF THE SYSTEM BOUNDARY (X = INCLUDED IN LCA; MND = MODULE OR INDICATOR NOT DECLARED; MNR
= MODULE NOT RELEVANT)
Benefits and
Construction loads beyond
Product stage Use stage End of life stage
process stage the system
boundaries
la ire ta m w a Ry lp p u s tro p s n a rT g n iru tc a fu n a M e h t m o rf tro p s n a rTe tis e h t o t e ta g y lb m e s s A e s U e c n a n e tn ia M ria p e R tn e m e c a lp e R tn e m h s ib ru fe R y g re n e la n o ita re p Oe s u re ta w la n o ita re p Oe s u n o itc u rts n o c -e Dn o itilo m e d tro p s n a rT g n is s e c o rp e ts a W la s o p s iD -e s u e R-y re v o c e R-g n ilc y c e Rla itn e to p
A1 A2 A3 A4 A5 B1 B2 B3 B4 B5 B6 B7 C1 C2 C3 C4 D
X X X MND MND MND MND MNR MNR MNR MND MND MND X X X X
RESULTS OF THE LCA - ENVIRONMENTAL IMPACT according to EN 15804+A2: 1 kg aluminium profiles
Parameter Unit A1-A3 C2 C3 C4 D
Global Warming Potential total (GWP-total) kg CO 2 eq 6.49E+00 1.2E-02 2.94E-01 5.91E-03 -6.27E+00
Global Warming Potential fossil fuels (GWP-fossil) kg CO 2 eq 6.29E+00 1.2E-02 2.92E-01 5.86E-03 -6.14E+00
Global Warming Potential biogenic (GWP-biogenic) kg CO 2 eq 4.12E-02 1.02E-05 1.9E-03 4.81E-05 -2.01E-02
Global Warming Potential luluc (GWP-luluc) kg CO 2 eq 1.66E-01 5.41E-06 2.59E-04 5.02E-06 -1.14E-01
Depletion potential of the stratospheric ozone layer (ODP) kg CFC11 eq 2.95E-07 2.55E-10 3.58E-09 7.89E-11 -1.32E-07
Acidification potential of land and water (AP) mol H+ eq 4.09E-02 2.41E-05 1.19E-03 3.23E-05 -4.47E-02
Eutrophication potential aquatic freshwater (EP-freshwater) kg P eq 1.8E-03 8.08E-07 6.99E-05 1.3E-06 -2.67E-03
Eutrophication potential aquatic marine (EP-marine) kg N eq 7.62E-03 6E-06 2.34E-04 9.19E-06 -6.01E-03
Eutrophication potential terrestrial (EP-terrestrial) mol N eq 6.38E-02 6.07E-05 2.55E-03 9.79E-05 -5.93E-02
kg NMVOC
Formation potential of tropospheric ozone photochemical oxidants (POCP) 2.49E-02 3.77E-05 8.52E-04 3.35E-05 -2.25E-02
eq
Abiotic depletion potential for non fossil resources (ADPE) kg Sb eq 1.46E-05 3.74E-08 6.05E-06 1.19E-08 4.73E-05
Abiotic depletion potential for fossil resources (ADPF) MJ 7.83E+01 1.65E-01 2.28E+00 7.98E-02 -7.49E+01
m3 world eq
Water use (WDP) 7.38E-01 6.33E-04 1.38E-02 1.56E-03 -9.78E-01
deprived
RESULTS OF THE LCA - INDICATORS TO DESCRIBE RESOURCE USE according to EN 15804+A2: 1 kg aluminium profiles
Parameter Unit A1-A3 C2 C3 C4 D
Renewable primary energy as energy carrier (PERE) MJ 4.75E+01 2.88E-03 2.32E-01 4.25E-03 -2.79E+01
Renewable primary energy resources as material utilization (PERM) MJ 5.57E-06 0 0 0 0
Total use of renewable primary energy resources (PERT) MJ 4.75E+01 2.88E-03 2.32E-01 4.25E-03 -2.79E+01
Non renewable primary energy as energy carrier (PENRE) MJ 7.83E+01 1.65E-01 2.28E+00 7.98E-02 -7.49E+01
Non renewable primary energy as material utilization (PENRM) MJ 0 0 0 0 0
Total use of non renewable primary energy resources (PENRT) MJ 7.83E+01 1.65E-01 2.28E+00 7.98E-02 -7.49E+01
Use of secondary material (SM) kg 5.37E-01 0 0 0 0
Use of renewable secondary fuels (RSF) MJ 0 0 0 0 0
Use of non renewable secondary fuels (NRSF) MJ 0 0 0 0 0
Use of net fresh water (FW) m3 5.39E-04 0 0 0 0
RESULTS OF THE LCA – WASTE CATEGORIES AND OUTPUT FLOWS according to EN 15804+A2:
1 kg aluminium profiles
Parameter Unit A1-A3 C2 C3 C4 D
Hazardous waste disposed (HWD) kg 3.24E-04 1.05E-06 5.95E-03 3.33E-07 6.81E-04
Non hazardous waste disposed (NHWD) kg 2.76E+00 6.8E-03 9.26E-01 2.06E-01 -1.61E+00
Radioactive waste disposed (RWD) kg 4.99E-04 6.53E-08 4.18E-06 7.03E-08 -1.94E-04
Components for re-use (CRU) kg 0 0 0 0 0
Materials for recycling (MFR) kg 3.59E-01 0 0 0 0
Materials for energy recovery (MER) kg 1.95E-02 0 0 0 0
Exported electrical energy (EEE) MJ 0 0 0 0 0
Exported thermal energy (EET) MJ 0 0 0 0 0
RESULTS OF THE LCA – additional impact categories according to EN 15804+A2-optional:
1 kg aluminium profiles
Parameter Unit A1-A3 C2 C3 C4 D
Disease
Incidence of disease due to PM emissions (PM) 5.66E-07 7.32E-10 2.1E-08 5.87E-10 -4.77E-07
incidence
Human exposure efficiency relative to U235 (IR) kBq U235 eq 1.89E+00 2.66E-04 1.65E-02 2.88E-04 -7.49E-01
Comparative toxic unit for ecosystems (ETP-fw) CTUe 2.62E+01 8.84E-02 2.67E+00 1.76E-01 -3.24E+00
Comparative toxic unit for humans (carcinogenic) (HTP-c) CTUh 2.43E-08 4.84E-12 1.91E-10 4.18E-12 -7.61E-09
Comparative toxic unit for humans (noncarcinogenic) (HTP-nc) CTUh 3.23E-07 1.4E-10 8E-09 1.21E-10 -2.21E-07
6 Environmental Product Declaration - Hilti Aktiengesellschaft - Aluminium profiles
Soil quality index (SQP) SQP 1.6E+01 8.45E-02 2.15E+00 9.56E-02 -3.99E+00
Disclaimer 1 – for the indicator “Potential Human exposure efficiency relative to U235”. This impact category deals mainly with the
eventual impact of low-dose ionizing radiation on human health of the nuclear fuel cycle. It does not consider effects due to possible
nuclear accidents, occupational exposure or radioactive waste disposal in underground facilities. Potential ionizing radiation from the
soil, radon and from some construction materials is also not measured by this indicator.
Disclaimer 2 – for the indicators “abiotic depletion potential for non-fossil resources”, “abiotic depletion potential for fossil resources”,
“water (user) deprivation potential, deprivation-weighted water consumption”, “potential comparative toxic unit for ecosystems”,
“potential comparative toxic unit for humans – cancerogenic”, “Potential comparative toxic unit for humans - not cancerogenic”,
“potential soil quality index”. The results of this environmental impact indicator shall be used with care as the uncertainties on these
results are high as there is limited experience with the indicator.
6. LCA: Interpretation
The LCA results are presented for 1 kg of aluminium profiles. responsible for 94 % of the total climate change impact
The charts below provide information on the impacts per main category.
processes of the upstream and manufacturing life cycle stages.
Based on the results it can be concluded that the dominant
material category appears to be materials responsible for 90 %
for the climate change category. The second biggest contributor
to the overall impact is disposal with 5 % for the climate change
category followed by the footprint of energy with a share of 3 %
for the climate change category.
In the figure below it can be seen that by excluding the final
disposal materials still represent the dominant category and are
7. Requisite evidence
The product is not a finished product (end product) and it is the design of the end product will vary, depending on the
used as raw material for other industries. The processing and application of the final product.
8. References
DIN EN 573-3:2019-10 assessment — Requirements and guidelines
Aluminium and aluminium alloys - Chemical composition and
form of wrought products - Part 3: Chemical composition and EN 15804
form of products EN 15804:2012+A2:2019+AC:2021, Sustainability of
construction works — Environmental Product Declarations —
DIN 4102-4 Core rules for the product category of construction products.
Fire behaviour of building materials and building components -
Part 4: Synopsis and application of classified building materials, ISO 45001
components and special components ISO 45001:2018 Occupational health and safety management
systems
ISO 9001 Further References
ISO 9001:2015 Quality management systems
BPR Regulation
ISO 14001 Biocidal Products Regulation EU 528/2012
ISO 14001:2015 Environmental management systems
European Aluminium Association
ISO 14025 A strategy for achieving aluminium's full potential for circular
EN ISO 14025:2011, Environmental labels and declarations — economy by 2030
Type III environmental declarations — Principles and https://european-
procedures. aluminium.eu/wpcontent/uploads/2022/08/european-aluminium-
circularaluminium-action-plan.pdf
ISO 14040
ISO 14040:2006, Environmental management — Life cycle ECHA list
assessment — Principles and framework List of substances of very high concern (SVHC) for
authorisation (ECHA Candidate List), 14.01.2020, published
ISO 14044 under Article 59(10) of REACH. Helsinki: European Chemicals
ISO 14044:2006, Environmental management — Life cycle Agency. http://echa.europa.eu/
7 Environmental Product Declaration - Hilti Aktiengesellschaft - Aluminium profiles
aluminium and aluminium alloys, v. 1.6
European Waste Catalogue (EWC)
Ordinance on the European Waste List (Waste List Ordinance Software and database
AVV) SimaPro
LCA and reporting softwareapps.simapro.com
IBU
Institut Bauen und Umwelt e.V.: General Instructions for the ecoinvent Version 3
EPD programme of Institut Bauen und Umwelt e.V., Version Wernet, G., Bauer, C., Steubing, B., Reinhard, J., Moreno-Ruiz,
2.0, Berlin: Institut Bauen und Umwelt e.V., 2021, E., and Weidema, B., 2016. The ecoinvent database version 3
www.ibuepd.com (part I): overview and methodology. The International Journal of
Life Cycle Assessment, [online] 21(9), pp.1218–1230.
PCR Part A: Calculation Rules for the Life Cycle Assessment The literature referred to in the Environmental Product
and Requirements on the Project Report according to Declaration must be listed in full.Standards already fully quoted
EN15804+A2:2019, v. 1.3 in the EPD do not need to be listed here again.
The current version of PCR Part A and PCR Part B of the PCR
PCR Part B: Requirements on the EPD for Products of document on which they are based must be referenced.
8 Environmental Product Declaration - Hilti Aktiengesellschaft - Aluminium profiles
Publisher
Institut Bauen und Umwelt e.V. +49 (0)30 3087748- 0
Hegelplatz 1 info@ibu-epd.com
10117 Berlin www.ibu-epd.com
Germany
Programme holder
Institut Bauen und Umwelt e.V. +49 (0)30 3087748- 0
Hegelplatz 1 info@ibu-epd.com
10117 Berlin www.ibu-epd.com
Germany
Author of the Life Cycle Assessment
denkstatt Bulgaria OOD +359 2 470 7508
Lyubata 4-6 office@denkstatt.bg
1407 Sofia http://denkstatt.bg/
Bulgaria
Owner of the Declaration
Hilti Aktiengesellschaft +423 234 2111
Feldkircher Strasse 100 HAGHSE@hilti.com
9494 Schaan www.hilti.com
Liechtenstein
9 Environmental Product Declaration - Hilti Aktiengesellschaft - Aluminium profiles
