ENVIRONMENTAL PRODUCT DECLARATION
as per ISO 14025 and EN 15804+A2
Owner of the Declaration Swisspearl Group AG
Publisher Institut Bauen und Umwelt e.V. (IBU)
Programme holder Institut Bauen und Umwelt e.V. (IBU)
Declaration number EPD-SWP-20230360-CCA1-EN
Issue date 24.10.2023
Valid to 23.10.2028
Slates
Swisspearl Group AG
www.ibu-epd.com | https://epd-online.com
General Information
Swisspearl Group AG Slates
Programme holder Owner of the declaration
IBU – Institut Bauen und Umwelt e.V. Swisspearl Group AG
Hegelplatz 1 Eternitstrasse 3
10117 Berlin 8867 Niederurnen
Germany Switzerland
Declaration number Declared product / declared unit
EPD-SWP-20230360-CCA1-EN 1m2 of Swisspearl Slates fibre cement board
This declaration is based on the product category rules: Scope:
Fibre cement / Fibre concrete, 01.08.2021 This declaration represents the production of 1 m² of Swisspearl Slates
(PCR checked and approved by the SVR) fibre cement board at the production site located in Beroun, Czech
Republic. Product specific data are based on production values from the
year 2021.
Issue date The owner of the declaration shall be liable for the underlying information
and evidence; the IBU shall not be liable with respect to manufacturer
24.10.2023
information, life cycle assessment data and evidences.
The EPD was created according to the specifications of EN 15804+A2. In
Valid to
the following, the standard will be simplified as EN 15804.
23.10.2028
Verification
The standard EN 15804 serves as the core PCR
Independent verification of the declaration and data according to ISO
14025:2011
internally X externally
Dipl.-Ing. Hans Peters
(Chairman of Institut Bauen und Umwelt e.V.)
Florian Pronold Dr. Matthew Fishwick,
(Managing Director Institut Bauen und Umwelt e.V.) (Independent verifier)
1 Environmental Product Declaration - Swisspearl Group AG - Slates
Product
The main constituents of Swisspearl Slates are as followed:
Product description/Product definition
• Portland cement: 75-80%
Swisspearl fibercement slates (4mm thickness) are
• Inert filler: 15-25%
manufactured using Portland cement together with a non-
• Cellulose: 2-4%
asbestos formulation of blended synthetic and cellulose fibres.
• Polyvinyl alcohol (PVA): 1-3%
The slates are fully compressed and are finished with a high
• Paint: 0-2%
quality, semi-matt acrylic coloured coating to the top face and
Material explanation
edges and a tinted or transparent, high performance binder to
the back face. • Portland Cement: Manufactured according to /DIN EN
This declaration is based on the average of various types of 197-1/ from limestone, marl and sand. The material is
slates produced in Beroun, Czech Republic. For the placing on crushed, dried, calcinated to clinker and ground to
the market of the product in the European Union/European cement.
Free Trade Association (EU/EFTA) (with the exception of • Inert filler: a filler to optimize deformation properties and
Switzerland) Regulation (EU) No. 305/2011 (CPR) applies. The material bonding.
product needs a declaration of performance taking into • Cellulose Fibres (0.5-3mm): To assure collection of
consideration EN492:2012+A2:2018/ and the CE marking. powder during filtration.
• PVA fibres (4-6mm): Synthetic Polyvinyl alcohol fibre
Application used as reinforcement.
The recommended use of Swisspearl Slates is as roofing (roof There are no substances of very high concern (SVHC) present
coverings) or cladding (internal and external wall finishes). in the product according to according to Regulation (EC)
No.1907/2006 (REACH)
Technical Data
The technical specifications of Swisspearl Slates can be seen Manufacturing
in the following table: Swisspearl Slates are manufactured with Hatschek technology.
Constructional data A very thin slurry of water, binder and fibres is mixed and
introduced into each of the vats of the Hatschek machine. The
Name Value Unit
rotating sieve cylinder in the vats collects a thin layer of solid
Thermal conductivity 0.3 - 0.4 W/(mK)
material that is further dewatered as it is transferred to a felt
Gross density ,dry min 1600 kg/m3 and further on to an accumulating format roller. At the required
Moisture content at 23 °C, 80% humidity 10 M.-% thickness, the accumulated layers are automatically cut into the
Coefficient of thermal expansion 10 10-6K-1 required product size, and transferred into the pre-curing area.
After pre-curing, the products are stored under continued
Bending moment 50 NM/m
control of temperature and humidity.
Additional data can be found on Swisspearl's webpage in either
the Declaration of Performance (DoP) or Safety Datasheets. Reference service life
There is no substantiated data on the reference service life
Performance data of the product is in accordance with the (RSL) of Swisspearl Slates. However, it is estimated that the
declaration of performance with respect to its essential RSL of Swisspearl Slates is 50 years or higher. This is in
characteristics according to EN 492:2012+A2:2018 'Fibre- accordance with the table published by the Bundesinstitut für
cement slates and fittings - Product specification and test Bau-, Stadt- und Raumforschung (BBSR) (code 335.511),
methods. which estimates the RSL of facade and roofing products from
fibrecement.
Base materials/Ancillary materials
LCA: Calculation rules
All slate variants have a thickness of 4 mm.
Declared Unit
In this EPD the declared unit is defined as the production of System boundary
1m2 of Swisspearl Slates with a thickness of 4mm, an expected The modules considered in this EPD follow a cradle-to-grave
lifetime of 50 years or higher, and its related impacts over the assessment: A1-A5, B1-B7, C1-C4, D.
'cradle to grave' life-cycle modules. A1 -The system boundary includes the provision and
processing of raw materials. These include in particular cement,
Declared unit and mass reference
plastic fibres, pulp and packaging materials.
Name Value Unit
Declared unit 1 m2 A2 -The transports to the manufacturer were specifically
Gross Density, dry min 1600 kg/m3 collected for all starting materials.
Grammage 9.2 kg/m2
A3 -The production includes all in-plant energy consumption
Layer thickness 0.004 m (gas + electricity), as well as water used in the production
Data is gathered at the production site in Beroun, Czech process, and production waste.
Republic for the year 2021. The weighted average based on the
total production volume is taken from all the types of slates A4 -The transport, part of the construction process, is an
produced at this site, including the RB/W02, RB/W03, RB/W04 average of the total distance of all products delivered to the
MS, and RB/W 05. Furthermore, these include painted and point of installation. This is calculated to be 1964 km.
dressed variants. Difference between the product variants are
considered to be small. A5 -All environmental impacts associated with the disposal of
2 Environmental Product Declaration - Swisspearl Group AG - Slates
packaging handled at the construction site are accounted for. It technological representativeness is considered to be good.
is assumed incinerated at an incineration plant. Furthermore,
environmental impacts associated with trucks and fuel for the Geographical: All primary and secondary data are collected
construction installation are included. specific to the countries/regions under study. Where
country/region-specific data are unavailable, proxy data are
B1-B7 modules are included, however, no significant used. The geographical representativeness is considered to be
environmental impact is associated with the use phase of the good.
product.
Temporal: All primary data collected is based on the year 2021.
C1 -Accounts for the environmental impacts associated with All secondary data come from the GaBi 2020.1 databases and
dismantling and demolition of the fibre cement boards. Fuel are representative for the years 2020-2025. Temporal
used for demolition equipment and transport on site vehicles. representativeness is considered to be very good.
C2 -Transportation of the discarded products from the Allocation in foreground data
construction site to a landfilling site. The transport is estimated The production process does not deliver any co-products.
to be 100 km in an average truck. Therefore, the applied model does not contain any allocation.
C3- The fibre cement boards are sent to landfill and therefore Allocation for waste materials
there are no environmental impacts associated with waste Pre-processing waste (plastics) is sent to a waste incineration
processing of materials flows intended for reuse, recycling or plant. The resulting electrical and thermal energy is credited in
energy recovery. module A1. For the waste incineration plant an R1-value of
above 0.6 is assumed.
C4 -Environmental impacts associated with the processes at
the landfill. Cut-off criteria
All raw materials used, utilized thermal energy, and electric
D -The fibre cement boards are sent to landfill after use. The power consumption of the production process are considered in
product has therefore no impact during this stage and no this assessment. This means that all material and energy flows
associated environmental impacts. The boards are expected to contributing less than 1% are considered.
be reusable over time, but this is not included in this
assessment. Incineration credits have been considered, and Geographic Representativeness
resulting credits for thermal and electrical energy are declared. Land or region, in which the declared product system is
manufactured, used or handled at the end of the product´s
Background data and data quality lifespan: Europe
Modelling of the production of 1m2 of Swisspearl Slates is done
with GaBi Software System and Database for Life Cycle
Comparability
Engineering. The model has been developed by Sphera
Basically, a comparison or an evaluation of EPD data is only
Solutions GmbH. Each background dataset has been reviewed
possible if all the data sets to be compared were created
on geographical, technological, and temporal scale.
according to EN 15804 and the building context, respectively
the product-specific characteristics of performance, are taken
Technological: All primary and secondary data are modelled to
into account. GaBi Software System and Database for Life
be specific to the technology mixes under study. Proxy data are
Cycle Engineering CUP Version: 2022.2
used where technology-specific data are unavailable. The
LCA: Scenarios and additional technical information
adding 100 km, representing the distance from the warehouse
Characteristic product properties of biogenic carbon to the installation point. Swisspearls' warehouses for which the
The biogenic carbon containing material (cellulose) in distance has been calculated are located in Denmark, Sweden,
Swisspearl Slates is required to be listed separately. The Norway, Netherlands, Belgium, Ireland and the United
following table shows the biogenic carbon content in the Kingdom.
product and accompanying packaging:
Name Value Unit
Information on describing the biogenic Carbon Content at Transport distance 1964 km
factory gate
Gross density of products transported 1850 kg/m3
Name ValueUnit
kg Installation into the building (A5)
Biogenic carbon content in product 0.016
C Installation of the boards is carried out by use of an automatic
Biogenic carbon content in accompanying kg screwdriver. The LCA model considers screws, however for
0.01
packaging C Swisspearl Slates, nails are commonly used. For the declared
unit of slates, 24 nails are used to mount. It is estimated that a
nail is half the size of a screw used to mount a roofing product.
Note: 1 kg of biogenic carbon is equivalent to 44/12 kg of CO .
2
PE film and wooden pallets are used as packaging materials.
Polyethylene foils can be recycled locally, and reusable pallets
can be returned to the building material suppliers.
Transport to the building site (A4) Name Value Unit
Estimating the transport to each individual construction site is Plastic waste 0.002 kg
rather complex. However, an educated estimate is made for the
Pallets 0.14 kg
distance to the installation point by averaging the total distance
Screws 12 pcs
of all products delivered to Swisspearls' warehouses and
3 Environmental Product Declaration - Swisspearl Group AG - Slates
.
End of life (C1-C4)
Reference service life Name Value Unit
Name ValueUnit Reuse - kg
Reference service life (according to ISO 15686-1, - Landfilling 9.2 kg
- a
2, -7 and -8)
Life Span (according to BBSR) >50 a
Life Span according to the manufacturer - a
4 Environmental Product Declaration - Swisspearl Group AG - Slates
LCA: Results
The following tables show the results of life-cycle assessment indicators, resource use and waste related to 1m2 of Swisspearl Slates.
The data is representative of the products of Swisspearl Group A/G.
DESCRIPTION OF THE SYSTEM BOUNDARY (X = INCLUDED IN LCA; MND = MODULE OR INDICATOR NOT DECLARED; MNR
= MODULE NOT RELEVANT)
Benefits and
Construction loads beyond
Product stage Use stage End of life stage
process stage the system
boundaries
la ire ta m w a Ry lp p u s tro p s n a rT g n iru tc a fu n a M e h t m o rf tro p s n a rTe tis e h t o t e ta g y lb m e s s A e s U e c n a n e tn ia M ria p e R tn e m e c a lp e R tn e m h s ib ru fe R y g re n e la n o ita re p Oe s u re ta w la n o ita re p Oe s u n o itc u rts n o c -e Dn o itilo m e d tro p s n a rT g n is s e c o rp e ts a W la s o p s iD -e s u e R-y re v o c e R-g n ilc y c e Rla itn e to p
A1 A2 A3 A4 A5 B1 B2 B3 B4 B5 B6 B7 C1 C2 C3 C4 D
X X X X X X X X X X X X X X X X X
RESULTS OF THE LCA - ENVIRONMENTAL IMPACT according to EN 15804+A2: 1 m^2 Swisspearl Slates
Parameter Unit A1 A2 A3 A4 A5 B1 B2 B3 B4 B5 B6 B7 C1 C2 C3 C4 D
GWP-total kg CO 2 6.28E 1.29E- 2.31E 1E+00 9.63E- 0 0 0 0 0 0 0 6.36E- 5.1E-02 -1.3E-01 6.04E- -7.99E-
eq +00 01 +00 01 04 01 02
GWP-fossil kg CO 2 6.27E 1.26E- 2.53E 9.57E- 7.05E- 0 0 0 0 0 0 0 6.3E-04 4.87E- 3.51E-01 1.21E- -7.94E-
eq +00 01 +00 01 01 02 01 02
GWP- kg CO 2 1.1E-02 3.53E- -2.17E- 4.41E- 2.58E- 0 0 0 0 0 0 0 5.35E- 2.24E- -4.82E- 4.82E- -3.85E-
biogenic eq 03 01 02 01 06 03 01 01 04
GWP-luluc kg CO 2 1.52E- 3.36E- 3.31E-04 2.27E- 5.49E- 0 0 0 0 0 0 0 8.92E- 1.16E- 8.6E-04 3.57E- -5.23E-
eq 03 05 05 04 07 06 04 05
kg CFC11 5.39E- 6.43E- 1.51E- 5.59E- 4.72E- -8.63E-
ODP 1.3E-14 8.14E-15 1.1E-16 0 0 0 0 0 0 0 1.15E-13
eq 16 15 17 18 16 16
1.13E- 1.26E- 7.87E- 1.59E- 1.31E- 4.01E- 8.65E- -1.01E-
AP mol H+ eq 2.86E-03 0 0 0 0 0 0 0 2.97E-03
02 03 04 03 06 05 04 04
EP- 3.71E- 8.15E- 2.03E- 1.42E- 1.69E- 1.04E- 2.04E- -9.89E-
kg P eq 3.6E-06 0 0 0 0 0 0 0 9.26E-06
freshwater 06 08 07 06 09 08 07 08
3.73E- 3.63E- 2.49E- 3.65E- 3.11E- 1.27E- 2.25E- -2.91E-
EP-marine kg N eq 7.96E-04 0 0 0 0 0 0 0 9.37E-04
03 04 04 04 07 05 04 05
4.09E- 3.98E- 2.76E- 3.94E- 3.27E- 2.47E- -3.12E-
EP-terrestrial mol N eq 8.48E-03 0 0 0 0 0 0 0 1.4E-04 9.88E-03
02 03 03 03 06 03 04
kg
1.17E- 1.02E- 7.52E- 1.14E- 8.45E- 3.83E- 6.81E- -8.18E-
POCP NMVOC 2.28E-03 0 0 0 0 0 0 0 2.67E-03
02 03 04 03 07 05 04 05
eq
2.79E- 9.96E- 3.34E- 2.86E- 1.85E- 1.15E- -1.28E-
ADPE kg Sb eq 1.68E-07 0 0 0 0 0 0 0 1.7E-09 1.16E-07
07 09 08 05 10 08 08
4.58E 3.38E 1.35E 7.37E 1.12E- 5.56E 1.61E -1.38E
ADPF MJ 1.8E+00 0 0 0 0 0 0 0 6.9E-01
+01 +01 +01 +00 02 +00 +00 +00
m3 world
2.54E- 3.71E- 1.59E- 6.14E- 1.01E- 8.07E- -5.79E-
WDP eq 6.26E-01 0 0 0 0 0 0 0 7.88E-03 1.3E-02
01 03 03 02 04 05 03
deprived
GWP = Global warming potential; ODP = Depletion potential of the stratospheric ozone layer; AP = Acidification potential of land and water; EP =
Eutrophication potential; POCP = Formation potential of tropospheric ozone photochemical oxidants; ADPE = Abiotic depletion potential for non-fossil
resources; ADPF = Abiotic depletion potential for fossil resources; WDP = Water (user) deprivation potential)
RESULTS OF THE LCA - INDICATORS TO DESCRIBE RESOURCE USE according to EN 15804+A2: 1 m^2 Swisspearl Slates
Parameter Unit A1 A2 A3 A4 A5 B1 B2 B3 B4 B5 B6 B7 C1 C2 C3 C4 D
-3.17E 1.85E- 3.69E 4.47E- 2.18E 5.16E- 2.27E- 1.51E 7.71E -2.97E-
PERE MJ 0 0 0 0 0 0 0
+00 01 +00 02 +00 03 03 +01 +00 01
7.49E -7.49E
PERM MJ 0 1.4E-01 0 -1.4E-01 0 0 0 0 0 0 0 0 0 0 0
+00 +00
4.32E 1.85E- 3.83E 4.47E- 2.04E 5.16E- 2.27E- 1.51E 2.17E- -2.97E-
PERT MJ 0 0 0 0 0 0 0
+00 01 +00 02 +00 03 03 +01 01 01
4.58E 3.34E 1.36E 7.74E 1.12E- 6.91E- 5.56E 1.61E -1.38E
PENRE MJ 1.8E+00 0 0 0 0 0 0 0
+01 +01 +01 +00 02 01 +00 +00 +00
PENRM MJ 0 0 3.4E-01 0 -3.4E-01 0 0 0 0 0 0 0 0 0 0 0 0
4.58E 3.38E 1.36E 1.12E- 6.91E- 5.56E 1.61E -1.38E
PENRT MJ 1.8E+00 7.4E+00 0 0 0 0 0 0 0
+01 +01 +01 02 01 +00 +00 +00
1.56E-
SM kg 0 1E-02 0 0 0 0 0 0 0 0 0 0 0 0 0 0
01
RSF MJ 0 0 0 0 0 0 0 0 0 0 0 0 0 0 0 0 0
NRSF MJ 0 0 0 0 0 0 0 0 0 0 0 0 0 0 0 0 0
1.26E- 1.84E- 1.82E- 7.18E- 2.88E- 5.03E- 3.65E- 3.91E- 3.98E-
FW m3 0 0 0 0 0 0 0 -2.9E-04
02 04 02 05 03 06 06 03 04
5 Environmental Product Declaration - Swisspearl Group AG - Slates
PERE = Use of renewable primary energy excluding renewable primary energy resources used as raw materials; PERM = Use of renewable primary
energy resources used as raw materials; PERT = Total use of renewable primary energy resources; PENRE = Use of non-renewable primary energy
excluding non-renewable primary energy resources used as raw materials; PENRM = Use of non-renewable primary energy resources used as raw
materials; PENRT = Total use of non-renewable primary energy resources; SM = Use of secondary material; RSF = Use of renewable secondary fuels;
NRSF = Use of non-renewable secondary fuels; FW = Use of net fresh water
RESULTS OF THE LCA – WASTE CATEGORIES AND OUTPUT FLOWS according to EN 15804+A2:
1 m^2 Swisspearl Slates
Parameter Unit A1 A2 A3 A4 A5 B1 B2 B3 B4 B5 B6 B7 C1 C2 C3 C4 D
1.14E- 6.96E- 9.33E- 1.19E- 2.96E- 4.75E- 6.97E- 1.71E- -3.07E-
HWD kg 5.3E-09 0 0 0 0 0 0 0
10 09 11 09 12 12 09 10 10
3.92E- 4.19E- 1.36E- 2.78E- 7.95E- 6.91E- 1.81E- 8.04E -6.23E-
NHWD kg 6.7E-01 0 0 0 0 0 0 0
02 04 03 02 06 05 02 +00 04
1.11E- 5.99E- 2.06E- 1.45E- 5.01E- 1.67E- 7.39E- 3.97E- 1.69E- -9.54E-
RWD kg 0 0 0 0 0 0 0
03 05 03 05 04 06 07 04 05 05
CRU kg 0 0 0 0 0 0 0 0 0 0 0 0 0 0 0 0 0
MFR kg 0 0 0 0 0 0 0 0 0 0 0 0 0 0 0 0 0
MER kg 0 0 0 0 0 0 0 0 0 0 0 0 0 0 0 0 0
1.98E-
EEE MJ 0 0 0 0 0 0 0 0 0 0 0 0 0 0 0 0
02
1.43E-
EET MJ 0 0 0 0 0 0 0 0 0 0 0 0 0 0 0 0
04
HWD = Hazardous waste disposed; NHWD = Non-hazardous waste disposed; RWD = Radioactive waste disposed; CRU = Components for re-use;
MFR = Materials for recycling; MER = Materials for energy recovery; EEE = Exported electrical energy; EET = Exported thermal energy
RESULTS OF THE LCA – additional impact categories according to EN 15804+A2-optional:
1 m^2 Swisspearl Slates
Parameter Unit A1 A2 A3 A4 A5 B1 B2 B3 B4 B5 B6 B7 C1 C2 C3 C4 D
Disease 1.38E- 2.02E- 5.06E- 4.38E- 1.82E- 2.23E- 1.88E- 1.07E-
PM 0 0 0 0 0 0 0 1.1E-11 -8.7E-10
incidence 07 08 08 09 08 10 07 08
kBq U235 1.72E- 1.42E- 2.06E- 7.32E- 2.74E- 1.05E- 6.46E- 1.78E- -1.56E-
IR 9.8E-03 0 0 0 0 0 0 0
eq 01 01 03 02 04 04 02 03 02
2.19E 1.18E 9.82E 2.39E 4.71E- 3.57E 9.19E- -2.75E-
ETP-fw CTUe 6.6E+00 0 0 0 0 0 0 0 5E-01
+01 +00 +00 +00 03 +00 01 01
8.89E- 2.36E- 1.83E- 5.91E- 1.33E- 1.88E- 1.35E-
HTP-c CTUh 2.8E-10 0 0 0 0 0 0 0 9.3E-12 -1.3E-11
10 11 10 10 13 10 10
8.84E- 1.01E- 2.19E- 7.63E- 7.61E- 5.03E- 3.89E- 1.18E- 1.49E- -5.13E-
HTP-nc CTUh 0 0 0 0 0 0 0
08 09 08 09 09 12 10 08 08 10
1.27E- 3.38E 3.47E- 1.56E 3.53E- 1.77E- 2.26E 3.25E- -2.03E-
SQP SQP 3.4E+00 0 0 0 0 0 0 0
01 +01 02 +00 03 03 +02 01 01
PM = Potential incidence of disease due to PM emissions; IR = Potential Human exposure efficiency relative to U235; ETP-fw = Potential comparative
Toxic Unit for ecosystems; HTP-c = Potential comparative Toxic Unit for humans (cancerogenic); HTP-nc = Potential comparative Toxic Unit for humans
(not cancerogenic); SQP = Potential soil quality index
Disclaimer 1 – for the indicator “Potential Human exposure efficiency relative to U235”. This impact category deals mainly with the
eventual impact of low-dose ionizing radiation on human health of the nuclear fuel cycle. It does not consider effects due to possible
nuclear accidents, occupational exposure or radioactive waste disposal in underground facilities. Potential ionizing radiation from the
soil, radon and from some construction materials is also not measured by this indicator.
Disclaimer 2 – for the indicators “abiotic depletion potential for non-fossil resources”, “abiotic depletion potential for fossil resources”,
“water (user) deprivation potential, deprivation-weighted water consumption”, “potential comparative toxic unit for ecosystems”,
“potential comparative toxic unit for humans – cancerogenic”, “Potential comparative toxic unit for humans - not cancerogenic”,
“potential soil quality index”. The results of this environmental impact indicator shall be used with care as the uncertainties on these
results are high as there is limited experience with the indicator.
This EPD was created using a software tool.
References
Standards ISO 15686-1, -2, -7 and -8
ISO 15686-1:2011
DIN EN 197-1 Part 1 General principles and framework
DIN EN 197-1, Cement - Part 1: Composition, specifications Part 2 Service life prediction procedures
and conformity criteria for common cements. Part 7 Performance evaluation for feedback of service life data
from practice
EN 492 Part 8 Reference service life and service-life estimation
EN 492:2012+A1, Fibre-cement slates and fittings — Product
specification and test methods. EN 15804
EN 15804:2012+A1:2013, Sustainability of construction works
ISO 14025 — Environmental Product Declarations — Core rules for the
EN ISO 14025:2011, Environmental labels and declarations — product category of construction products.
Type III environmental declarations — Principles and
procedures. EN 15804
EN 15804:2012+A2:2019+AC:2021, Sustainability of
6 Environmental Product Declaration - Swisspearl Group AG - Slates
construction works — Environmental Product Declarations — EPD programme of Institut Bauen und Umwelt e.V., Version
Core rules for the product category of construction products. 2.0,Berlin: Institut Bauen und Umwelt e.V., 2021 www.ibu-
epd.com
REACH
Regulation (EC) No 1907/2006, Registration, Evaluation, PCR Part A
Authorisation and Restriction of Chemicals (REACH) Calculation Rules for the Life Cycle Assessment and
Requirements on the Project Report,Berlin: Institut Bauen und
Further References Umwelt e.V., www.ibu-epd.com, Version 2.2, 2022
BBSR PCR Part B
Bundesinstitut für Bau-, Stadt- und Raumforschung Requirements of the EPD for Fibre Cement/Fibre Concrete,
(BBSR): Nutzungsdauer von Bauteilen für version 1.7, Institut Bauen und Umwelt e.V., www.bau-
Lebenszyklusanalyse nach Bewertungssystem umwelt.com, 2019
Nachhaltiges Bauen (BNB), 2011
REGULATION (EU) No 305/2011 Harmonised conditions for
GaBi documentation the marketing of construction products and repealing Council
GaBi life cycle inventory data documentation Directive 89/106/EEC
www.gabisoftware.com/support/gabi/gabidatabase2020lcidocumentation
Swisspearl Group A/G
GaBi software Swisspearl Group A/G: Information on technical data and
Sphera Solutions GmbH downloads.
GaBi Software System and Database for Life Cycle Downloads - Swisspearl
Engineering
CUP Version: 2022.2 The literature referred to in the Environmental Product
University of Stuttgart Declaration must be listed in full.Standards already fully quoted
Leinfelden Echterdingen in the EPD do not need to be listed here again.
The current version of PCR Part A and PCR Part B of the PCR
IBU 2021 document on which they are based must be referenced.
Institut Bauen und Umwelt e.V.: General Instructions for the
7 Environmental Product Declaration - Swisspearl Group AG - Slates
Publisher
Institut Bauen und Umwelt e.V. +49 (0)30 3087748- 0
Hegelplatz 1 info@ibu-epd.com
10117 Berlin www.ibu-epd.com
Germany
Programme holder
Institut Bauen und Umwelt e.V. +49 (0)30 3087748- 0
Hegelplatz 1 info@ibu-epd.com
10117 Berlin www.ibu-epd.com
Germany
Author of the Life Cycle Assessment
Sphera Solutions GmbH +49 711 341817-0
Hauptstraße 111- 113 info@sphera.com
70771 Leinfelden-Echterdingen www.sphera.com
Germany
Owner of the Declaration
Swisspearl Group AG +41 56 617 11 11
Eternitstrasse 3 eco@swisspearl.ch
8867 Niederurnen www.swisspearl.ch
Switzerland
8 Environmental Product Declaration - Swisspearl Group AG - Slates
