ENVIRONMENTAL PRODUCT DECLARATION
as per ISO 14025 and EN 15804+A2
Owner of the Declaration Grundfos Holding A/S
Publisher Institut Bauen und Umwelt e.V. (IBU)
Programme holder Institut Bauen und Umwelt e.V. (IBU)
Declaration number EPD-GRU-20240014-CBA1-EN
Issue date 21.03.2024
Valid to 20.03.2029
MAGNA3 65-40/60 (Stainless Steel)
Grundfos Holding A/S
www.ibu-epd.com | https://epd-online.com
General Information
Grundfos Holding A/S MAGNA3 65-40/60 (Stainless Steel)
Programme holder Owner of the declaration
IBU – Institut Bauen und Umwelt e.V. Grundfos Holding A/S
Hegelplatz 1 Poul Due Jensens Vej 7
10117 Berlin 8850 Bjerringbro
Germany Denmark
Declaration number Declared product / declared unit
EPD-GRU-20240014-CBA1-EN 1 PCS. of MAGNA3 65-40/60 (Stainless Steel)
This declaration is based on the product category rules: Scope:
Pumps for liquids and liquids with solids, 01.08.2021 The declaration applies to 1 piece of MAGNA3 (Stainless Steel) pump.
(PCR checked and approved by the SVR)
The product is produced in Wahlstedt, Germany, and the life cycle
assessment is based on data collected at the production site.
Issue date
Production has been modeled using annual production data from 2021.
21.03.2024
The declaration covers two different types of the MAGNA3 65- product
(40/60).
Valid to
20.03.2029 The owner of the declaration shall be liable for the underlying information
and evidence; the IBU shall not be liable with respect to manufacturer
information, life cycle assessment data and evidences.
The EPD was created according to the specifications of EN 15804+A2. In
the following, the standard will be simplified as EN 15804.
Verification
The standard EN 15804 serves as the core PCR
Independent verification of the declaration and data according to ISO
14025:2011
Dipl.-Ing. Hans Peters internally X externally
(Chairman of Institut Bauen und Umwelt e.V.)
Florian Pronold Mrs Kim Allbury,
(Managing Director Institut Bauen und Umwelt e.V.) (Independent verifier)
1 Environmental Product Declaration - Grundfos Holding A/S - MAGNA3 65-40/60 (Stainless Steel)
Product
Product description/Product definition Standard: EN 50581:2012.
The Grundfos MAGNA3 circulator pumps are designed for
circulating liquids in heating systems, air conditioning and Ecodesign Directive (2009/125/EC)
cooling systems and domestic hot water systems. However, the
pump range can also be used in ground source heat pump Commission Regulation (EC) No: 641/2009 and
systems and solar heating systems.
Commission Regulation (EU) 622/2012
The MAGNA3 pump is a centrifugal pump powered by an
electrical motor. It has a high-performance neodymium magnet Standards used:
rotor which increases motor efficiency and an insulation shell to EN 16297-1:2012, EN 16297-2:2012, EN 16297-3:2012.
reduce heat loss from the cast iron pump housing with threaded
connections. The CE marking takes into account the proof of conformity with
the respective harmonized norms based on the legal provisions
The declaration covers two types of the MAGNA3 pump. They above.
are grouped as shown below. The group reference in the
technical data and scenarios refers also to these. MAGNA3 pumps are not harmonized in accordance with the
CPR.
GROUP 1 - MAGNA3 65-40
Application
GROUP 2 - MAGNA3 65-60 For the application and use the respective national provisions
apply.
These are all the same physical products and 100 % identical
in terms of design, dimensions and materials as well as supply The pump is designed for circulating liquids in the following
chain and manufacturing processes, i.e., all cradle to gate systems:
processes (A1-A3).
· heating systems
The products are also identical in terms of packaging,
distribution, reference service life and end-of-life treatment. · domestic hot-water systems
The only thing that differentiates the products from each other · air-conditioning and cooling systems
is the software which controls how the pump operates in the
system in which it is installed, making them fit for different · ground-source heat-pump systems
applications. Hence, all life cycle modules are identical, except
use stage module B6, which will change, as the applied · solar-heating systems
scenarios for electricity consumption changes. For the placing
on the market in the European Union/European Free Trade The pump is suitable for thin, clean, non-aggressive and non-
Association (EU/EFTA) (with the exception of Switzerland) the explosive liquids, not containing solid particles or fibres that
following legal provisions apply: may attack the pump mechanically or chemically. In heating
systems, the water must meet the requirements of accepted
Machinery Directive (2006/42/EC) standards on water quality in heating systems. The pumps are
also suitable for domestic hot-water systems.
Standard used: EN 809:1998 + A1:2009.
Technical Data
Radio Equipment Directive (2014/53/EU) The performance data of the product according to the
harmonised norms, based on the harmonisation
Standards used: provisions above apply. The relevant technical specifications
EN 60335-1:2012/AC:2014 + A11:2014, EN 60335-2-51:2003 + according to the PCR Part B are given in the table below.
A1:2008 + A2:2012, EN 62233:2008. Characteristics that are the same for all two product groups are
only given once. Others are given individually for all groups.
EN 55014-1:2006 Constructional data
A1:2009 + A2:2011, EN 55014-1:2017, EN 61000-6-2:2005, EN
61000-3-2:2014, EN 61000-3-3:2013, ETSI EN 301 489-1
V2.2.0, ETSI EN 301 489-17 V3.2.0. ETSI EN 300 328 V2.1.1
Electromagnetic Compatibility (EMC) Directive
(2014/30/EU)
Standards used:
EN 55014-1:2017, EN 55014-2:2015,
EN 61000-3-2:2014/2019, EN 61000-6-2:2008/2019,
EN 61000-3-3:2013 A1:2019
RoHS Directive 2011/65/EU and 2015/863//EU
2 Environmental Product Declaration - Grundfos Holding A/S - MAGNA3 65-40/60 (Stainless Steel)
Name Value Unit
This product/article/at least one partial article contains
Frequency 50 Hz
substances listed in the ECHA candidate list (date:10.06.2022)
Voltage 230 V
exceeding 0.1 percentage by mass: no
Clean
Pumped liquid (e.g. water) -
Water
Energy Efficiency Index Gr.1 0,18 The Wahlstedt production has been assessed and certified as
Energy Efficiency Index Gr.2 0,17 meeting the requirements in ISO 14001, ISO 50001, ISO 45001
Flow range Gr. 1 (max) 23,0 m3/h and ISO 9001.
Flow range Gr. 2 (max) 32,0 m3/h
Head max. Gr.1 4 m
Head max. Gr. 2 6 m
Reference service life
Power input Gr. 1 Average (from load profile
0,109 m No use stage scenario which refers to the lifetime of the product
describing use)
is declared. However, to facilitate building calculations, an
Power input Gr. 2 Average (from load profile
0,155 m estimated RSL of 10 years can be used. This is an EU
describing use)
consensus-based estimation, referenced on page 37 in
Nominal capacity Gr.1 0,19 kW Appendix 7: Lot 11 – Circulators in Buildings, prepared by AEA
Nominal capacity Gr.2 0,342 kW Energy & Environment for the European Commission in the
context of the Eco Design Directive:
Performance data of the product according to the harmonised
standards, based on provisions for harmonisation.
There is no definitive information on the average circulator life
Base materials/Ancillary materials available, there is consensus within the industry that it is at
least 12 years. However, this is complicated by many factors,
Base materials / Ancillary materials
including many being scrapped prematurely when e.g. the
Name Value Unit boiler they are connected to is replaced.
Aluminium 13 %
Ceramics 0,29 % From the estimated stock (140Mpa) and annual sales (14Mpa),
the average lifetime of the circulator is taken as 10 years for the
Copper 2,43 %
purposes of this study.
Electronics 0,22 %
Magnet Nd 1,04 % The RSL of the declared product is not directly influencing the
Paper 0,48 % results in this study, as no declared use stage scenario is
PCB 3,57 % dependent on the RSL; The use stage sub-module B6 is
declared per year as required by the PCR Part B.
Plastics 0,31 %
Plastics, foam 1,17 %
Plastics GF 4,93 %
Rubber 0,16 %
Stainless steel 59,97 %
Steel 4,85 %
Cardboard 7,64 %
Plastic film 0,07 %
TOTAL 100 %
REACH
LCA: Calculation rules
and processing, transport processes as well as the
Declared Unit manufacturing process. The final production and assembly of
The declared the MAGNA3 pump takes place at a Grundfos manufacturing
unit is 1 piece (pcs.) of MAGNA3 (Stainless Steel) pump. site in Germany. However, the full supply-chain leading to the
Declared unit finished product at the gate is rather complex and includes a
large amount of raw materials, components and semi-finished
Name Value Unit
parts which comes from both external suppliers as well as other
Declared unit 1 pce.
Grundfos production facilities.
Mass reference 24.1 kg/pce
Conversion factor [Mass/Declared Unit] 24.1 The product stage is included in the study, and according to EN
15804 the system boundary with nature is set to include those
System boundary processes that provide the material and energy inputs into the
system and the following manufacturing, transport up to the
This EPD is Cradle-To-Grave. The system boundaries of the
factory gate as well as the processing any waste arising from
EPD follow the modular approach in EN 15804. By decision no.
those processes.
20170712-n of the SVR, the modules B3, B4 and B5 are by
default declared as "MNR" (module not relevant).
Wastes and losses are included in the modules where they
occur according to the polluter pays principle and the modular
The product stage (A1-A3) comprises raw material extraction
3 Environmental Product Declaration - Grundfos Holding A/S - MAGNA3 65-40/60 (Stainless Steel)
approach of EN 15804. According to European statistics, the average R1 value of
incineration plants is > 0.6. Therefore, it is assumed that
The product includes: packaging material is treated thermally in an incineration plant
with R1 > 0.6. The loads from the combustion process of
· A1 Extraction and processing of raw materials; packaging are declared in module A5 and the resulting energy
benefits in module D, as required by the PCR Part A, 5.5.2.
· A1 Reuse of products or materials from a previous product
system; Use stage (B1-B7):
· A1 Processing of secondary materials; The use stage, related to the building fabric includes:
· A1 Generation of electricity, steam and heat from primary · B1, use or application of the installed product;
energy resources, also including their extraction, refining and
transport; · B2, maintenance.
· A1 Energy recovery and other recovery processes from The use stage related to the operation of the building includes:
secondary fuels;
· B6, operational energy use;
· A2 Transportation up to the factory gate and internal transport;
· B7, operational water use.
· A3 Production of ancillary materials or pre products;
In this study, all use stage modules are assessed, though B1,
· A3 Manufacturing of products and coproducts; B2 and B7 are assessed to be zero. By decision no. 20170712-
n of the SVR, the modules B3, B4 and B5 are by default
· A3 Manufacturing of packaging; declared as "MNR" (module not relevant).
· A1-A3 processing up to the end-of-waste state or disposal of The modules include the provision and transport of all
final residues. materials, products and related energy and water use, as well
as waste processing up to the end-of-waste state or disposal of
For secondary material inputs, the system boundary to the final residues during the use stage. They also include all
previous system (providing the secondary material) is set where impacts and aspects related to the losses during the use stage
outputs reach the end-of-waste state. The recycling of (i.e. production, transport, and waste processing and disposal
secondary material into new raw materials is included in the of the lost products and materials).
system boundary of this study. Waste materials from production
processes that are recycled without any modification of the Generally, the geographical coverage of the datasets used
material's inherent characteristics are modelled as closed-loop matches the actual processes taking place. Meaning, that when
within A1-A3. This is done up to the input mass flow that was modelling taking place in Grundfos Bjerringbro, the Danish
used during production. electricity grid mix is used in the model and thermal energy
from natural gas. These are generally of very high quality with
Waste for incineration arising in the product stage is accounted very good technological, temporal and geographical
for in the module where the waste is produced. The representativeness.
environmental loads from the incineration process are declared
in the module where it occurs and the electricity and heat which Contributions to operational energy use during the use stage
is produced from the incineration are considered as closed-loop (B6) come from the electricity consumption of the product. The
within A1-A3, as described in PCR Part A, 5.5.1. The input of annual electricity consumption is calculated by multiplying the
biogenic carbon from the production of packaging material is average power input, which is based on a defined load profile,
inventoried in A3. As required by PCR Part A, the with the annual running hours. For use stage (B6) European
corresponding end-of-life module of the packaging material, A5, Average electricity grid mix has been used. These values are
is also declared and the emissions of biogenic carbon are declared in the scenarios section.
inventoried.
The End-of-Life stage (C1-C4) includes all activities from
The construction process stage (A4-A5) includes: when the product reaches the end of its service life and no
longer provides any functionality and until all materials and
· A4: Transportation from factory gate to the distribution center: components are processed for reuse/recycling or disposed of.
· Consumption of electricity, thermal energy and water at the According to EN 15804 and the PCR Part A, the end-of-life
distribution center; stage includes:
· Transportation from distribution center to construction site; · C1 deconstruction of the product from the building, including
initial on-site sorting of the materials;
· Wastage during distribution.
· C2 transportation of the discarded product to a recycling site
· A5: Installation process; and transportation of waste to final disposal;
· Transport of packaging waste to treatment site; · C3 waste processing, collection of waste fractions from the
deconstruction and waste processing of material flows intended
· Waste treatment of packaging. for reuse, recycling and energy recovery;
The packaging material does not reach the end of waste state · C4 waste disposal including physical pretreatment and
but is incinerated as waste. management of the disposal site.
4 Environmental Product Declaration - Grundfos Holding A/S - MAGNA3 65-40/60 (Stainless Steel)
potentials, expressed as net impacts and benefits. Any
At the end of life, the MAGNA3 pump is manually disassembled declared benefits and loads from net
from the piping system in which it has been installed. The
definition of the applied end-of-life scenario in this EPD follows flows leaving the product system that have not been allocated
the requirements in the PCR Part A, 6.2 regarding complex as co-products and that have passed the end-of-waste state
products, with a combination of recycling, thermal waste are included in module D.
treatment and landfilling. 100 % of the material is considered in
the end of life scenario as required by the PCR. An overall Contributions to module D comes from waste incineration
collection rate of 90 % has been assumed. processes in A5 and C3 as well as material recycling in C3. The
specific fractions and net flows are shown in the scenarios
Materials from which energy is recovered in an incineration section.
process with an R1-value above 0.60 are in this study included
with the environmental burdens from the incineration process Geographic Representativeness
inventoried in C3, the recovered energy is declared as exported Land or region, in which the declared product system is
energy in C3 manufactured, used or handled at the end of the product´s
lifespan: Europe
and the energy benefits are declared in D. This procedure is
according to the PCR Part A, 5.5.6. C3 includes the mechanical
Comparability
separation of the product followed by a series of sorting steps.
Basically, a comparison or an evaluation of EPD data is only
Metal fractions are recycled and plastics, cardboard and
possible if all the data sets to be compared were created
electronics are assumed incinerated with energy recovery. The
according to EN 15804 and the building context, respectively
residual fractions are landfilled and declared in C4.
the product-specific characteristics of performance, are taken
into account. Software and databases used: LCA for Experts
The specific amounts are shown in the scenarios section.
10.7.1.28
Schema 8007
Beyond system boundary (D): According to EN 15804
Sphera and Ecoinvent databases
module D includes the reuse, recovery and/or recycling
LCA: Scenarios and additional technical information
referenced in Appendix 7: Lot 11 – Circulators in Buildings,
Characteristic product properties of biogenic carbon prepared by AEA Energy & Environment for the European
The biogenic carbon content quantifies the amount of biogenic Commission in the context of the Eco Design Directive.
carbon in a construction product leaving the factory gate, and it
Reference service life
will be separately declared for the product and for any
accompanying packaging, as required from the PCR Part A. Name Value Unit
The Carbon content of Cardboard and Paper is assumed to Life Span according to the manufacturer 10 a
0.46 kg C. It means 46% of the paper and carbdoard is
assumed to be biogenic carbon content. Overall, there is an Operational energy use (B6)
amount of weight-% Carbon in the product leaving the factory Name Value Unit
gate and has to be considered Electricity consumption Group 1 545 kWh/a
Electricity consumption Group 2 775 kWh/a
Information on describing the biogenic Carbon Content at Average power input, Group 1 0,109 kW
factory gate
Average power input, Group 2 0,155 kW
Name ValueUnit
Running hours (all groups) 5.000 h/a
Biogenic carbon content in accompanying kg
0.9
packaging C End of life (C1-C4)
Note: 1 kg of biogenic carbon is equivalent to 44/12 kg of CO2 Name Value Unit
Collected as mixed construction waste 22,125 kg
Transportation distance (C2) 500 km
Aluminium for recycling 2,74 kg
Transport from the gate to the site (A4) Steel for recycling 1,03 kg
Name Value Unit Copper for recycling 0,52 kg
Litres of fuel 0,0332 l/100km Stainless steel for recycling 12,75 kg
Transport distance 2003 km Plastics for incineration w/energy 1,40 kg
Capacity utilisation (including empty runs) 85 % Electronics for incineration w/energy 0,80 kg
Gross density of products transported 445 kg/m3 Landfilling 2,89 kg
Wastage during distribution 0,02 %
Reuse, recovery and/or recycling potentials (D), relevant
Installation into the building (A5) scenario information
Name ValueUnit
Packaging waste for incineration (LDPE film) 0,016 kg
Packaging waste for incineration
1,955 kg
(Paper/Cardboard)
An estimated RSL of 10 years can be used to facilitate building
calculations. This is an EU consensus-based estimation,
5 Environmental Product Declaration - Grundfos Holding A/S - MAGNA3 65-40/60 (Stainless Steel)
Name Value Unit
A5, incineration w/energy recov. thermal energy 8,9 MJ
A5, incineration w/energy recov. electric energy) 4,92 MJ
C3, steel for recycling (net amounts) -0,93 kg
C3, stainless steel for recycling (net amounts) 3,92 kg
C3, aluminium for recycling (net amounts) -0,433 kg
C3, copper for recycling (net amounts) 0,221 kg
C3, incineration w/energy recov. thermal energy 13,4 MJ
C3, incineration w/energy recov. electric energy 7,45 MJ
6 Environmental Product Declaration - Grundfos Holding A/S - MAGNA3 65-40/60 (Stainless Steel)
LCA: Results
Characterization model: EN 15804 - 2012+A2 - 2019, PEF. By Decision no. 20170712-n of the IBU SVR, the modules B3, B4, B5 are
marked as MNR (module not relevant) as default. The LCA results in module B6 are given on a period of one year, according to PCR
Part B. To obtain the results from module B6 over the entire life cycle, the LCA results of module B6 must be multiplied by the
estimated RSL of 10 years. The indicator results for module B6 are declared for Group 1. B6 indicator results for other groups can be
derived by multiplying the B6 indicator results with the following factors:
Group 2: 1,422
DESCRIPTION OF THE SYSTEM BOUNDARY (X = INCLUDED IN LCA; MND = MODULE OR INDICATOR NOT DECLARED; MNR
= MODULE NOT RELEVANT)
Benefits and
Construction loads beyond
Product stage Use stage End of life stage
process stage the system
boundaries
la ire ta m w a Ry lp p u s tro p s n a rT g n iru tc a fu n a M e h t m o rf tro p s n a rTe tis e h t o t e ta g y lb m e s s A e s U e c n a n e tn ia M ria p e R tn e m e c a lp e R tn e m h s ib ru fe R y g re n e la n o ita re p Oe s u re ta w la n o ita re p Oe s u n o itc u rts n o c -e Dn o itilo m e d tro p s n a rT g n is s e c o rp e ts a W la s o p s iD -e s u e R-y re v o c e R-g n ilc y c e Rla itn e to p
A1 A2 A3 A4 A5 B1 B2 B3 B4 B5 B6 B7 C1 C2 C3 C4 D
X X X X X X X MNR MNR MNR X X X X X X X
RESULTS OF THE LCA - ENVIRONMENTAL IMPACT according to EN 15804+A2: 1PCS of MAGNA3 65-40/60
Parameter Unit A1 A2 A3 A4 A5 B1 B2 B6 B7 C1 C2 C3 C4 D
GWP-total kg CO 2 eq 1.17E+02 6.06E+00 6.92E-01 1.85E+00 3.17E+00 0 0 1.77E+02 0 0 7.6E-01 6.25E+00 1.42E-01 -1.13E+01
GWP-fossil kg CO 2 eq 1.17E+02 6.06E+00 3.91E+00 1.86E+00 4.69E-01 0 0 1.76E+02 0 0 7.64E-01 6.24E+00 1.44E-01 -1.13E+01
GWP- -3.25E
biogenic kg CO 2 eq -1.7E-02 -9.06E-03 +00 -2.73E-02 2.7E+00 0 0 1.53E+00 0 0 -1.13E-02 1.54E-02 -1.78E-03 -3.31E-02
GWP-luluc kg CO 2 eq 7.29E-02 8.8E-03 3.04E-02 1.68E-02 9.56E-05 0 0 1.91E-02 0 0 7.09E-03 2.27E-04 1.3E-04 -2.44E-03
kg CFC11
ODP 4.74E-08 4.73E-13 4.06E-09 1.07E-11 4.18E-13 0 0 3.24E-09 0 0 9.97E-14 3.34E-11 2.4E-13 -2.61E-11
eq
AP mol H+ eq 8.51E-01 1.82E-01 1.94E-02 1.11E-02 8.61E-04 0 0 3.76E-01 0 0 4.6E-03 4.61E-03 4.44E-04 -1.08E-01
EP-
kg P eq 1.52E-03 4.6E-06 6.86E-05 6.98E-06 1.56E-07 0 0 6.56E-04 0 0 2.8E-06 9.46E-06 1.66E-05 -1.52E-05
freshwater
EP-marine kg N eq 9.23E-02 4.33E-02 4.06E-03 5.34E-03 3.15E-04 0 0 8.98E-02 0 0 2.24E-03 1.2E-03 1.06E-04 -1.26E-02
EP-terrestrial mol N eq 9.93E-01 4.75E-01 4.07E-02 5.92E-02 3.96E-03 0 0 9.39E-01 0 0 2.49E-02 1.34E-02 1.16E-03 -1.36E-01
kg
POCP NMVOC 2.93E-01 1.23E-01 1.14E-02 1.02E-02 8.19E-04 0 0 2.4E-01 0 0 4.25E-03 3.2E-03 3.34E-04 -4.04E-02
eq
ADPE kg Sb eq 8.86E-03 1.09E-07 6.05E-05 1.9E-06 4.31E-09 0 0 2.72E-05 0 0 5.08E-08 2.79E-07 3.87E-09 -1.22E-03
ADPF MJ 1.64E+03 7.54E+01 5.8E+01 2.54E+01 1.16E+00 0 0 3.7E+03 0 0 1.04E+01 3.89E+01 2.15E+00 -1.34E+02
m3 world
WDP eq 3.91E+01 1.99E-02 3.94E-02 3.11E-02 3.81E-01 0 0 3.92E+01 0 0 9.25E-03 8.52E-01 -2E-03 -7.15E-01
deprived
GWP = Global warming potential; ODP = Depletion potential of the stratospheric ozone layer; AP = Acidification potential of land and water; EP =
Eutrophication potential; POCP = Formation potential of tropospheric ozone photochemical oxidants; ADPE = Abiotic depletion potential for non-fossil
resources; ADPF = Abiotic depletion potential for fossil resources; WDP = Water (user) deprivation potential)
RESULTS OF THE LCA - INDICATORS TO DESCRIBE RESOURCE USE according to EN 15804+A2: 1PCS of MAGNA3 65-40/60
Parameter Unit A1 A2 A3 A4 A5 B1 B2 B6 B7 C1 C2 C3 C4 D
PERE MJ 4.28E+02 1.21E+00 5.58E+01 1.97E+00 2.62E-01 0 0 2.21E+03 0 0 7.59E-01 2.27E+01 1.94E-01 2.42E+00
PERM MJ 0 0 0 0 0 0 0 0 0 0 0 0 0 0
PERT MJ 4.28E+02 1.21E+00 5.58E+01 1.97E+00 2.62E-01 0 0 2.21E+03 0 0 7.59E-01 2.27E+01 1.94E-01 2.42E+00
-1.34E
PENRE MJ 1.64E+03 7.56E+01 5.8E+01 2.55E+01 1.16E+00 0 0 3.7E+03 0 0 1.05E+01 3.89E+01 2.15E+00
+02
PENRM MJ 0 0 0 0 0 0 0 0 0 0 0 0 0 0
-1.34E
PENRT MJ 1.64E+03 7.56E+01 5.8E+01 2.55E+01 1.16E+00 0 0 3.7E+03 0 0 1.05E+01 3.89E+01 2.15E+00
+02
SM kg 1.45E+01 0 2.31E-01 2.94E-03 0 0 0 0 0 0 0 0 0 0
RSF MJ 1.46E-23 0 0 2.91E-27 0 0 0 0 0 0 0 0 0 0
NRSF MJ 1.71E-22 0 0 3.42E-26 0 0 0 0 0 0 0 0 0 0
FW m3 1.16E+00 1.38E-03 2.32E-02 2.26E-03 8.99E-03 0 0 1.79E+00 0 0 8.32E-04 2.88E-02 2.25E-05 2.19E-02
PERE = Use of renewable primary energy excluding renewable primary energy resources used as raw materials; PERM = Use of renewable primary
energy resources used as raw materials; PERT = Total use of renewable primary energy resources; PENRE = Use of non-renewable primary energy
excluding non-renewable primary energy resources used as raw materials; PENRM = Use of non-renewable primary energy resources used as raw
materials; PENRT = Total use of non-renewable primary energy resources; SM = Use of secondary material; RSF = Use of renewable secondary fuels;
7 Environmental Product Declaration - Grundfos Holding A/S - MAGNA3 65-40/60 (Stainless Steel)
NRSF = Use of non-renewable secondary fuels; FW = Use of net fresh water
RESULTS OF THE LCA – WASTE CATEGORIES AND OUTPUT FLOWS according to EN 15804+A2:
1PCS of MAGNA3 65-40/60
Parameter Unit A1 A2 A3 A4 A5 B1 B2 B6 B7 C1 C2 C3 C4 D
HWD kg 7.01E-06 2.37E-10 1.21E-04 2.57E-08 2.94E-11 0 0 4.35E-07 0 0 3.24E-11 4.42E-09 1.8E-10 -2.44E-03
NHWD kg 9.22E+00 7.69E-03 3.75E-01 5.94E-03 1.23E-01 0 0 2.71E+00 0 0 1.6E-03 6.46E-01 2.49E+00 2.02E+00
RWD kg 5.6E-02 9.78E-05 1.78E-03 6.33E-05 5.29E-05 0 0 5.88E-01 0 0 1.96E-05 6.03E-03 2.53E-05 -2.62E-03
CRU kg ND ND ND ND ND ND ND ND ND ND ND ND ND ND
MFR kg 0 0 0 0 0 0 0 0 0 0 0 1.7E+01 0 0
MER kg ND ND ND ND ND ND ND ND ND ND ND ND ND ND
EEE MJ 0 0 0 0 4.92E+00 0 0 0 0 0 0 7.45E+00 0 0
EET MJ 0 0 0 0 8.9E+00 0 0 0 0 0 0 1.34E+01 0 0
HWD = Hazardous waste disposed; NHWD = Non-hazardous waste disposed; RWD = Radioactive waste disposed; CRU = Components for re-use;
MFR = Materials for recycling; MER = Materials for energy recovery; EEE = Exported electrical energy; EET = Exported thermal energy
RESULTS OF THE LCA – additional impact categories according to EN 15804+A2-optional:
1PCS of MAGNA3 65-40/60
Parameter Unit A1 A2 A3 A4 A5 B1 B2 B6 B7 C1 C2 C3 C4 D
Disease
PM 1.07E-05 3.15E-06 2.88E-07 7.2E-08 5.08E-09 0 0 3.16E-06 0 0 2.92E-08 3.91E-08 4.51E-09 -2.69E-06
incidence
kBq U235
IR 7.52E+00 1.41E-02 2.85E-01 9.35E-03 8.26E-03 0 0 9.79E+01 0 0 2.92E-03 1E+00 3.74E-03 -2.26E-01
eq
ETP-fw CTUe 8.32E+02 5.34E+01 1.98E+01 1.79E+01 5.59E-01 0 0 1.03E+03 0 0 7.47E+00 1.12E+01 1.35E+00 -1.65E+01
HTP-c CTUh 2.38E-05 9.92E-10 6.46E-07 5.26E-09 3.05E-11 0 0 5.44E-08 0 0 1.52E-10 6.24E-10 8.68E-11 -5.35E-07
HTP-nc CTUh 1.76E-06 3.4E-08 4.24E-08 1.64E-08 1.14E-09 0 0 8.68E-07 0 0 6.75E-09 1.25E-08 7.41E-09 -7.13E-08
SQP SQP 3.81E+02 5.56E+00 1.06E+02 1.05E+01 3.41E-01 0 0 1.45E+03 0 0 4.36E+00 1.51E+01 1.92E-01 -1.75E+01
PM = Potential incidence of disease due to PM emissions; IR = Potential Human exposure efficiency relative to U235; ETP-fw = Potential comparative
Toxic Unit for ecosystems; HTP-c = Potential comparative Toxic Unit for humans (cancerogenic); HTP-nc = Potential comparative Toxic Unit for humans
(not cancerogenic); SQP = Potential soil quality index
Disclaimer 1 – for the indicator 'Potential Human exposure efficiency relative to U235'.
This impact category deals mainly with the eventual impact of low-dose ionizing radiation on human health of the nuclear fuel cycle. It
does not consider effects due to possible nuclear accidents, occupational exposure or radioactive waste disposal in underground
facilities. Potential ionizing radiation from the soil, radon and from some construction materials is also not measured by this indicator.
Disclaimer 2 – for the indicators 'abiotic depletion potential for non-fossil resources', 'abiotic depletion potential for fossil resources',
'water (user) deprivation potential, deprivation-weighted water consumption', 'potential comparative toxic unit for ecosystems', 'potential
comparative toxic unit for humans – cancerogenic', 'Potential comparative toxic unit for humans - not cancerogenic', 'potential soil
quality index'. The results of this environmental impact indicator shall be used with care as the uncertainties on these results are high
as there is limited experience with the indicator.
Disclaimer 3: JRC Technical Reports, Version 2, 2018 Page 6, for the indicator "EP-freshwater". This indicator has been calculated as
'kg P eq' as required in the characterization model EUTREND model, Struijs et al., 2009b, as implemented in ReCiPe; This EPD was
created using a software tool.
References
Standards PARLIAMENT AND OF THE COUNCIL of 26 February
Machinery Directive 2014 on the harmonistion of the laws of the Member
DIRECTIVE 2006/42/EC OF THE EUROPEAN States relating to electromagnetic compatibility
PARLIAMENT AND OF THE COUNCIL of 17 May Ecodesign Directive
2006 on machinery DIRECTIVE 2009/125/EC OF THE EUROPEAN
Radio Equipment Directive PARLIAMENT AND OF THE COUNCIL of 21 October
DIRECTIVE 2014/53/EU OF THE EUROPEAN PARLIAMENT 2009 establishing a framework for the setting of
AND OF THE COUNCIL of 16 April 2014 on the harmonisation
of the laws of the Member States relating to the making ecodesign requirements for energy-related products
available on the market of
EC 641/2009
radio equipment
COMMISSION REGULATION (EC) No 641/2009 of 22 July
Electromagnetic Compatibility (EMC) Directive 2009 implementing Directive 2005/32/EC of the European
Parliament and of the Council with regard to ecodesign
DIRECTIVE 2014/30/EU OF THE EUROPEAN requirements for glandless standalone circulators and
glandless circulators integrated in
8 Environmental Product Declaration - Grundfos Holding A/S - MAGNA3 65-40/60 (Stainless Steel)
EN 50581:2012
products
EN 50581:2012, Technical documentation for the
EC 622/2012
assessment of electrical and electronic products with
COMMISSION REGULATION (EU) No 622/2012 of 11 July
2012 amending Regulation (EC) No 641/2009 with regard to respect to the restriction of hazardous substances
ecodesign requirements for glandless standalone circulators
and glandless circulators integrated in products EN 60335-1
DIRECTIVE 2011/65/EU EN 60335-1:2012/A11:2014/A13:2017, Household
DIRECTIVE 2011/65/EU OF THE EUROPEAN and similar electrical appliances – Safety – Part 1:General
requirements
PARLIAMENT AND OF THE COUNCIL of 8 June 2011
EN 60335-2-51
on the restriction of the use of certain hazardous
EN 60335-2-51:2003-03 + A1:2008 + A2:2012, Household and
substances in electrical and electronic equipment similar electrical appliances – Safety –Part 2-51: Particular
requirements for stationary circulation pumps for heating and
DIRECTIVE 2015/863/EU service water installations
DIRECTIVE 2015/863/EU of 31 March 2015 amending EN 61000-3-2
Annex II to Directive 2011/65/EU of the European EN 61000-3-2:2014/2019, Electromagnetic compatibility (EMC)
– Part 3-2: Limits – Limits for harmonic current emissions
Parliament and of the Council as regards the list of (equipment input current =16 A per phase)
restricted substances EN 61000-3-3
ETSI EN 301 489-1 EN 61000-3-3:2013-08/ A1:2019, Electromagnetic compatibility
(EMC) – Part 3-3:
ETSI EN 301 489-1 V2.2.0, Electromagnetic Compatibility Limits – Limitation of voltage changes, voltage fluctuations and
(EMC) standard for radio equipment and services; Part 1: flicker in public low voltage supply systems, for equipment with
Common technical requirements
rated current <= 16 A per phase and not subject to conditional
ETSI EN 301 489-17 connection
ETSI EN 301 489-17 V3.2.0, Electromagnetic Compatibility EN 61000-6-2
(EMC) standard for radio equipment and services; Part 17:
Specific conditions for Broadband Data Transmission Systems EN 61000-6-2:2008/2019, Electromagnetic compatibility (EMC)
– Part 6-2: Generic standards –Immunity for industrial
ETSI EN 300 328 V2.1.1 environments
ETSI EN 300 328 V2.1.1, Wideband transmission systems; EN 16297-1
Data transmission equipment operating in the 2,4 GHz ISM
band and using wide band modulation techniques EN 16297-1:2012-10, Pumps – Rotodynamic pumps –
Glandless circulators – Part 1:
EN 809 General requirements and procedures for testing and
calculation of energy efficiency index (EEI)
EN 809:1998-10 + A1:2009, Pumps and pump units for
EN 16297-2
liquids - Common safety requirements
EN 16297-2:2012-10, Pumps – Rotodynamic pumps –
EN 55014-1 Glandless circulators – Part 2: Calculation of energy efficiency
index (EEI) for standalone circulators
EN 55014-1:2017, Electromagnetic compatibility –
Requirements for household appliances, electric tools and EN 16297-3
similar apparatus – Part 1: Emission
EN 16297-3:2012, Pumps – Rotodynamic pumps –Glandless
EN 55014-2 circulators – Part 3: Energy efficiency index (EEI) for circulators
integrated in products
EN 55014-2:2015, Electromagnetic compatibility –
ISO 14001
Requirements for household appliances, electric tools
EN ISO 14001:2015-09, Environmental management systems -
and similar apparatus – Part 2: Immunity – Product Requirements with guidance for use
family standard (CISPR 14-2:2015) ISO 14025
9 Environmental Product Declaration - Grundfos Holding A/S - MAGNA3 65-40/60 (Stainless Steel)
DIN EN /ISO 14025:2011-10, Environmental labels and
declarations — Type III environmental declarations — Impact assessment characterization factors Institute of
Principles and procedures Environmental Sciences, Leiden University, Netherlands
EN 15804 ECHA candidate list
EN 15804:2012-04+A1 2013, Sustainability of construction Candidate List of substances of very high concern (SVHCs) for
works — Environmental Product Declarations — Core rules for authorisation, European Chemicals Agency (ECHA), Helsinki,
the product category of construction products Finland EUTREND model
Struijs et al., 2009b
PCR Part A
AEA Energy & Environment
Institut Bauen und Umwelt e.V., Berlin (pub.): Product Category Circulators in Buildings
Rules for Building-Related Products and Services, Product
Category Rules for Construction Products from the range of Ecoinvent
Environmental Product Declarations of Institut Bauen und
Umwelt (IBU), Part A: Calculation Rules for the Life Cycle Ecoinvent v3.9.1
Assessment and Requirements on the Project Report, Version
1.3. LCA for Experts
PCR Part B 10.7.1.28 Schema 8007 REACH
Institut Bauen und Umwelt e.V., Berlin (pub.): Product Category Regulation (EC) No 1907/2006 of the European Parliament and
Rules for Building-Related Products and Services, Product of the Council of 18 December 2006 concerning the
Category Rules for Construction Products from the range of Registration, Evaluation, Authorisation and Restriction of
Environmental Product Declarations of Institut Bauen und Chemicals (REACH) (Status: 27.06.2018)
Umwelt (IBU), Part B: Requirements on the EPD for Pumps for
liquids and liquids with solids, Version 1.0 (2018) SVR
Further references Advisory Board (formerly SVA)
CPR Decision no.
20170712-n
REGULATION (EU) No 305/2011 OF THE EUROPEAN The literature referred to in the Environmental Product
PARLIAMENT AND OF THE COUNCIL of 9 March 2011 laying Declaration must be listed in full.Standards already fully quoted
down harmonised conditions for the marketing of construction in the EPD do not need to be listed here again.
products and repealing Council Directive 89/106/EEC The current version of PCR Part A and PCR Part B of the PCR
document on which they are based must be referenced.
CML 2001
10 Environmental Product Declaration - Grundfos Holding A/S - MAGNA3 65-40/60 (Stainless Steel)
Publisher
Institut Bauen und Umwelt e.V. +49 (0)30 3087748- 0
Hegelplatz 1 info@ibu-epd.com
10117 Berlin www.ibu-epd.com
Germany
Programme holder
Institut Bauen und Umwelt e.V. +49 (0)30 3087748- 0
Hegelplatz 1 info@ibu-epd.com
10117 Berlin www.ibu-epd.com
Germany
Author of the Life Cycle Assessment
Grundfos Holding A/S +4587501400
Poul Due Jensens Vej 7 LCA_EPD@grundfos.com
8850 Bjerringbro www.grundfos.com
Denmark
Owner of the Declaration
Grundfos Holding A/S +4587501400
Poul Due Jensens Vej 7 LCA_EPD@grundfos.com
8850 Bjerringbro www.grundfos.com
Denmark
11 Environmental Product Declaration - Grundfos Holding A/S - MAGNA3 65-40/60 (Stainless Steel)
