ENVIRONMENTAL PRODUCT DECLARATION
as per ISO 14025 and EN 15804+A2
Owner of the Declaration Fletco Carpets A/S
Publisher Institut Bauen und Umwelt e.V. (IBU)
Programme holder Institut Bauen und Umwelt e.V. (IBU)
Declaration number EPD-FLE-20230272-CBC2-EN
Issue date 25/07/2023
Valid to 24/07/2028
Woven carpet tiles, pile material PET, print design, maximum total
pile weight 700 g/m², TEXtile backing
Fletco Carpets A/S
www.ibu-epd.com | https://epd-online.com
General Information
Fletco Carpets A/S Woven carpet tiles, pile material PET, print design,
maximum total pile weight 700 g/m², TEXtile
backing
Programme holder Owner of the declaration
IBU – Institut Bauen und Umwelt e.V. Fletco Carpets A/S
Hegelplatz 1 Mads Clausens Vej 2
10117 Berlin 7441 Bording
Germany Denmark
Declaration number Declared product / declared unit
EPD-FLE-20230272-CBC2-EN 1 m2 woven TEXtile carpet having a pile material of
Polyethylenterephthalate (PET).
This declaration is based on the product category rules: Scope:
Floor coverings, 01/08/2021 The manufacturer declaration applies to a group of products with a
(PCR checked and approved by the SVR) maximum total pile weight of 700 g/m2.
LCA results for products of the same construction but with a maximum total
pile weight of 400 g/m2 can be taken from the corresponding tables of the
Issue date annexe. Specific data for every product within the declared group of
25/07/2023 products in relation to its total pile weight can be calculated by using
equation 1 given in the annexe (see annexe chapter: 'General Information
on the annexe').
Valid to Weaving and dyeing of the carpet tiles takes place at the Fletco
manufacturing site Bording, Denmark and pre-coating and backing are
24/07/2028 performed at the Foamtex site, Bording, Denmark.
The declaration is only valid in conjunction with a valid GUT-PRODIS
license of the specific product.
The owner of the declaration shall be liable for the underlying information
and evidence; the IBU shall not be liable with respect to manufacturer
information, life cycle assessment data and evidences.
The EPD was created according to the specifications of EN 15804+A2. In
the following, the standard will be simplified as EN 15804.
Verification
The standard EN 15804 serves as the core PCR
Dipl.-Ing. Hans Peters
(Chairman of Institut Bauen und Umwelt e.V.) Independent verification of the declaration and data according to ISO
14025:2011
internally X externally
Florian Pronold Angela Schindler,
(Managing Director Institut Bauen und Umwelt e.V.) (Independent verifier)
1 Environmental Product Declaration - Fletco Carpets A/S - Woven carpet tiles, pile material PET, print design, maximum total pile weight 700 g/m², TEXtile backing
Product
Performance data of the product in accordance with the
Product description/Product definition declaration of performance with respect to its essential
Flat woven carpet tiles having a pile material of characteristics according to EN 14041: 2018-05, Resilient,
polyethylenterephthalate (PET) and a TEXtile backing. The textile and laminate floor coverings - Essential characteristics.
TEXtile backing includes a polyethylene-based heavy backing Additional product properties in accordance with EN 1307 can
and a felt backing made of 100 % recycled PET. be found on the Product Information System PRODIS using the
The recycled content out of total weight amounts to a minimum PRODIS registration number of the product (www.pro-dis.info)
14.5 %. or on the manufacturer's technical information section.
The injection printing dyeing method allows the creation of
various designs. Base materials/Ancillary materials
The declaration applies to a group of products with a maximum Name Value Unit
total pile weight of 700 g/m2. The LCA results are calculated for Polyethylenterephthalate (PET) 43,8 %
products with the maximum total pile weight.
Polymer dispersion (solid content) 8.0 %
LCA results for products with a maximum total pile weight of
Mineral filler 23.2 %
400 g/m2 can be taken from the corresponding tables of the
Aluminium hydroxide 6.4 %
annexe. Results for specific products with any other total pile
weight can be calculated by using equation 1 given in the Low-density polyethylene 17.5 %
annexe (see annexe chapter: 'General Information on the Glass fibre 1.0 %
annexe'). Additives 0.1 %
For the placing on the market of the specific product in the
The specific product covered by the EPD contains substances
European Union/European Free Trade Association (EU/EFTA)
listed in the ECHA candidate list (26.07.2022) or other
(with the exception of Switzerland) Regulation (EU) No.
carcinogenic, mutagenic or reprotoxic (CMR) substances in
305/2011 Construction Product Regulation (CPR) applies. The
categories 1A or 1B which are not on the candidate list
product needs a Declaration of Performance (DoP) taking into
exceeding 0.1 percentage by mass: no
consideration EN 14041:2018-05, Resilient, textile and laminate
The products are registered in the GUT-PRODIS Information
floor coverings - Essential characteristics, and the CE-marking.
System. The PRODIS system ensures compliance with
The DoP of the product can be found on the manufacturer's
limitations of various chemicals and Volatile Organic Compound
technical information section. For the application and use of the
(VOC)-emissions and a ban on the use of all substances that
product the respective national provisions apply.
are listed as 'Substances of Very High Concern' (SVHC) under
Application REACH.
According to the use class as defined in EN 1307 the products
Reference service life
can be used in all professional areas with heavy use which
The service life of textile floor coverings strongly depends on
require class 33 or less.
the correct installation taking into account the declared use
classification and the adherence to cleaning and maintenance
instructions.
A calculation of the reference service life according to ISO
15686 is not possible. Alternatively, a reference service life of
Technical Data 10 years can be assumed, during which the functional and
visual quality is guaranteed (BNB, Nutzungsdauer von
Bauteilen). The technical service life can be significantly longer.
Constructional data according to EN 1307
Name Value Unit
Product Form Tiles 50 cm x 50 cm -
Type of
Woven carpet -
manufacture
Dyeing method Injection printing method -
Yarn type Polyethylenterephthalate (PET) -
Secondary TEXtiles (heavy tile backing with a
-
backing recycled PET felt)
Total pile weight
700 g/m²
max.
Total carpet
3440 g/m2
weight max.
LCA: Calculation rules
Name Value Unit
Declared Unit
Declared unit 1 m2
Grammage 3.44 kg/m2
Layer thickness 0.005 m
Gross density 680 kg/m3
2 Environmental Product Declaration - Fletco Carpets A/S - Woven carpet tiles, pile material PET, print design, maximum total pile weight 700 g/m², TEXtile backing
The declared unit refers to 1 m2 produced textile floor covering. The modules are not relevant within the assumed reference
The Output of module A5 'Assembly' is 1 m2 installed textile service life of 10 years.
floor covering.
B6 - B7:
No energy and water input are required for the operation of the
carpet in the use stage. The modules are not relevant and not
System boundary declared.
Type of EPD:
Cradle-to-gate with options, modules C1-C4, module D, and C1 De-construction:
additional modules A4, A5, B1, B2. The floor covering is de-constructed manually and no additional
environmental impact is caused.
System boundaries of modules A, B, C, D:
Modules C3, C4 and D are indicated separately for three end- C2 Transport:
of-life scenarios: Transport of the carpet waste to a landfill, to the municipal
1 - landfill disposal waste incineration plant (MWI) or to the waste collection facility
2 - municipal waste incineration for recycling.
3 - recovery in a cement plant
C3 Waste processing:
A1-A3 Production: C3-1: Landfill disposal needs no waste processing.
Energy supply and production of the basic material, processing C3-2: Impact from waste incineration (plant with R1>0.6),
of secondary material, auxiliary material, transport of the generated electricity and steam are listed in the result table as
material to the manufacturing site, emissions, waste water exported energy.
treatment, packaging material and waste processing up to the C3-3: Collection of the carpet waste for recovery in the cement
landfill disposal of residual waste (except radioactive waste). industry, waste processing (granulating), transport to the
Benefits for generated electricity and steam due to the cement plant, emissions from the incineration.
incineration of production waste are aggregated.
C4 Disposal:
A4 Transport: C4-1: Impact from landfill disposal,
Transport of the packed textile floor covering from factory gate C4-2: The carpet waste leaves the system in module C3-2,
to the place of installation. C4-3: The pre-processed carpet waste leaves the system in
module C3-3.
A5 Installation:
Installation of the textile floor covering, processing of D Recycling potential:
installation waste and packaging waste up to the landfill Calculated benefits result from materials exclusive secondary
disposal of residual waste (except radioactive waste), the materials (net materials).
production of the amount of carpet that occurs as installation D-A5: Benefits for generated energy due to incineration of
waste including its transport to the place of installation. packaging and installation waste (incineration plant with R1 >
Generated electricity and steam due to the incineration of 0.6),
waste are listed in the result table as exported energy. D-1: Benefits for generated energy due to landfill disposal of
Preparation of the floor and auxiliary materials (adhesives, carpet waste at the end of life,
fixing agents, PET connectors) are beyond the system D-2: Benefits for generated energy due to incineration of carpet
boundaries and not taken into account. waste at the end-of-life (incineration plant with R1 > 0.6),
D-3: Benefits for saved fossil energy and saved inorganic
B1 Use: material due to recovery of the carpet in a cement plant.
Indoor emissions during the use stage. After the first year, no
Geographic Representativeness
product-related Volatile Organic Compound (VOC) emissions
are relevant due to known VOC decay curves of the product. Land or region, in which the declared product system is
manufactured, used or handled at the end of the product´s
B2 Maintenance: lifespan: Europe
Cleaning of the textile floor covering for a period of 1 year:
Vacuum cleaning – electricity supply
Comparability
Wet cleaning – electricity, water consumption, production of the
Basically, a comparison or an evaluation of EPD data is only
cleaning agent, waste water treatment.
possible if all the data sets to be compared were created
The declared values in this module have to be multiplied by the
according to EN 15804 and the building context, respectively
assumed service life of the floor covering in the building in
the product-specific characteristics of performance, are taken
question.
into account. Background data are taken from the GaBi
database 2022-2.
B3 - B5:
LCA: Scenarios and additional technical information
Characteristic product properties of biogenic carbon
Name ValueUnit
Transport to the construction site (A4)
Biogenic carbon content in accompanying kg
0.04
packaging at factory gate C
1 kg of biogenic carbon is equivalent to 44/12 kg of CO .
2
3 Environmental Product Declaration - Fletco Carpets A/S - Woven carpet tiles, pile material PET, print design, maximum total pile weight 700 g/m², TEXtile backing
Name Value Unit End of Life (C1-C4)
Litres of fuel (truck, EURO 0-6 mix) 0.0081 l/100km Three different end-of-life scenarios are declared and the
Transport distance 700 km results are indicated separately in module C.
Capacity utilisation (including empty runs) 55 % Each scenario is calculated as a 100 % scenario.
Scenario 1: 100 % landfill disposal
Gross density of products transported 680 kg/m3
Scenario 2: 100 % municipal waste incineration (MWI)
with R1>0.6
Installation in the building (A5)
Scenario 3: 100 % recovery in the cement industry
Name Value Unit
Material loss 0.103 kg If combinations of these scenarios have to be calculated this
Cardboard packaging waste is considered to be recycled. should be done according to the following scheme:
Preparation of the floor and auxiliaries (adhesives, fixing EOL-impact = x % impact (Scenario 1)
agents, PET connectors etc.) are not taken into account. + y % impact (Scenario 2)
+ z % impact (Scenario 3)
with x % + y % + z % = 100 %
Maintenance (B2)
Name ValueUnit
The values for cleaning refer to 1 m2 floor covering per year.
Collected as mixed construction waste (scenarios 1
Depending on the application based on ISO 10874, the 3.44 kg
and 2)
technical service life recommended by the manufacturer and
the anticipated strain on the floor by customers, the case- Collected separately waste type (scenario 3) 3.44 kg
specific useful life can be established. Based on this useful life Landfilling (scenario 1) 3.44 kg
the effects of module B2 need to be calculated in order to Energy recovery (scenario 2) 3.44 kg
obtain the overall environmental impacts.
Energy recovery (scenario 3) 2.387 kg
Name Value Unit
Recycling (scenario 3) 1.053 kg
Maintenance cycle (vacuum cleaning) 208 Number /year
Maintenance cycle (wet cleaning) 1,5 Number /year
Reuse, recovery and/or recycling potentials (D), relevant
Water consumption (wet cleaning) 0.004 m3 scenario information
Cleaning agent (wet cleaning) 0.09 kg Recovery or recycling potentials due to the three end-of-life
Electricity consumption 0.314 kWh scenarios (module C) are indicated separately.
For further information on cleaning and maintenance see
Recycling in the cement industry (scenario 3)
www.fletcocarpets.com
The organic material of the carpet is used as an alternative fuel
in a cement kiln. It mainly substitutes for lignite (68.8 %), hard
coal (23.6 %) and petrol coke (7.6 %). The inorganic material is
Service life substantially integrated into the cement clinker and substitutes
Name Value Unit for original material input. VDZ e.V.
Life Span (according to BBSR) 10 a
Corresponds to the
Declared product properties (at
specifications of EN -
the gate) and finishes
1307
An assumed quality of work,
Conforms to the
when installed in accordance
manufacturer's -
with the manufacturer’s
instructions
instructions
Usage conditions, e.g. Use in areas defined by
frequency of use, mechanical the use class according -
exposure to EN 1307
Maintenance e.g. required According to the
frequency, type and quality and manufacturer's -
replacement of components instructions
4 Environmental Product Declaration - Fletco Carpets A/S - Woven carpet tiles, pile material PET, print design, maximum total pile weight 700 g/m², TEXtile backing
LCA: Results
The declared result figures in module B2 have to be multiplied by the assumed service life (in years) of the floor covering in the building
under consideration.
Information on non-relevant modules:
Modules B3 - B7 are not relevant during the service life of the carpet.
Modules C3/1, C4/2 and C4/3 cause no additional impact (see chapter "LCA: Calculation rules" in this document).
Module C2 represents the transport for scenarios 1, 2 and 3. The values in column D result from module A5 (incineration of installation
waste).
DESCRIPTION OF THE SYSTEM BOUNDARY (X = INCLUDED IN LCA; ND = MODULE OR INDICATOR NOT DECLARED; MNR =
MODULE NOT RELEVANT)
Benefits and
Construction loads beyond
Product stage Use stage End-of-life stage
process stage the system
boundaries
la ire ta m w a Ry lp p u s tro p s n a rT g n iru tc a fu n a M e h t m o rf tro p s n a rTe tis e h t o t e ta g y lb m e s s A e s U e c n a n e tn ia M ria p e R tn e m e c a lp e R tn e m h s ib ru fe R y g re n e la n o ita re p Oe s u re ta w la n o ita re p Oe s u n o itc u rts n o c -e Dn o itilo m e d tro p s n a rT g n is s e c o rp e ts a W la s o p s iD -e s u e R-y re v o c e R-g n ilc y c e Rla itn e to p
A1 A2 A3 A4 A5 B1 B2 B3 B4 B5 B6 B7 C1 C2 C3 C4 D
X X X X X X X MNR MNR MNR MND MND X X X X X
RESULTS OF THE LCA - ENVIRONMENTAL IMPACT according to EN 15804+A2: 1 m² floor covering
Parameter Unit A1-A3 A4 A5 B1 B2 C1 C2 C3/2 C3/3 C4/1 D D/1 D/2 D/3
-1.66E
GWP-total kg CO 2 eq 9.24E+00 2.1E-01 6.19E-01 0 5.49E-01 0 1.17E-02 6.09E+006.14E+00 2.41E-01 -4.98E-02 0 +00 -3.79E-01
-1.65E
GWP-fossil kg CO 2 eq 9.32E+00 2.06E-01 4.69E-01 0 3.48E-01 0 1.15E-02 6.09E+006.14E+00 2.41E-01 -4.95E-02 0 +00 -3.79E-01
GWP-
biogenic kg CO 2 eq -8.15E-02 2.67E-03 1.5E-01 0 4.16E-03 0 1.48E-04 3.87E-04 9.17E-04 -3.96E-08 -2.52E-04 0 -8.41E-03 -4.35E-04
GWP-luluc kg CO 2 eq 3.55E-03 1.17E-03 1.48E-04 0 1.96E-01 0 6.49E-05 1.12E-04 2.78E-04 1.19E-04 -5.42E-06 0 -1.81E-04 -1.79E-04
kg CFC11
ODP 3.04E-11 1.25E-14 9.23E-13 0 3.42E-08 0 6.98E-16 3.4E-13 5.99E-13 3.28E-13 -3.33E-13 0 -1.11E-11 -5.99E-13
eq
AP mol H+ eq 1.53E-02 1.25E-03 5.27E-04 0 8.32E-04 0 6.93E-05 9.11E-04 1.12E-03 7.23E-04 -6.49E-05 0 -2.16E-03 -1.31E-03
EP-
kg P eq 2.06E-05 6.25E-07 6.5E-07 0 5.19E-06 0 3.48E-08 4.1E-07 5.48E-07 4.55E-05 -6.77E-08 0 -2.26E-06 -4.2E-07
freshwater
EP-marine kg N eq 4.77E-03 6.12E-04 1.72E-04 0 1.97E-04 0 3.4E-05 2.89E-04 3.83E-04 1.6E-04 -1.76E-05 0 -5.88E-04 -4.13E-04
EP-terrestrial mol N eq 5.16E-02 6.77E-03 1.89E-03 0 2.83E-03 0 3.77E-04 4.2E-03 5.23E-03 1.75E-03 -1.89E-04 0 -6.3E-03 -4.52E-03
kg
POCP NMVOC 1.6E-02 1.16E-03 5.42E-04 4.18E-04 9.83E-04 0 6.43E-05 7.92E-04 9.76E-04 5.14E-04 -4.94E-05 0 -1.65E-03 -1.25E-03
eq
ADPE kg Sb eq 1.27E-06 1.75E-08 3.9E-08 0 2.3E-07 0 9.73E-10 1.47E-08 2.19E-08 1.69E-08 -7.44E-09 0 -2.48E-07 -3.61E-08
-2.81E -5.06E
ADPF MJ 2.18E+02 2.8E+00 6.67E+00 0 5.9E+00 0 1.56E-01 1.61E+002.32E+00 3.46E+00 -8.42E-01 0
+01 +01
m3 world
WDP eq 1.79E+00 1.87E-03 7.33E-02 0 9.99E-02 0 1.04E-04 6.48E-01 6.52E-01 -2.59E-03 -5.19E-03 0 -1.73E-01 -5.71E-02
deprived
GWP = Global warming potential; ODP = Depletion potential of the stratospheric ozone layer; AP = Acidification potential of land and water; EP =
Eutrophication potential; POCP = Formation potential of tropospheric ozone photochemical oxidants; ADPE = Abiotic depletion potential for non-fossil
resources; ADPF = Abiotic depletion potential for fossil resources; WDP = Water (user) deprivation potential)
RESULTS OF THE LCA - INDICATORS TO DESCRIBE RESOURCE USE according to EN 15804+A2: 1 m² floor covering
Parameter Unit A1-A3 A4 A5 B1 B2 C1 C2 C3/2 C3/3 C4/1 D D/1 D/2 D/3
PERE MJ 3.23E+01 1.59E-01 1.17E+00 0 3.69E+00 0 8.85E-03 3.39E-01 5.39E-01 2.84E-01 -2.3E-01 0 -7.66E+00 -5.05E-01
PERM MJ 1.85E-01 0 -1.85E-01 0 0 0 0 0 0 0 0 0 0 0
PERT MJ 3.25E+01 1.59E-01 9.89E-01 0 3.69E+00 0 8.85E-03 3.39E-01 5.39E-01 2.84E-01 -2.3E-01 0 -7.66E+00 -5.05E-01
PENRE MJ 1.62E+02 2.81E+00 6.68E+00 0 5.9E+00 0 1.56E-01 5.78E+01 5.85E+01 3.46E+00 -8.42E-01 0 -2.81E+01-5.06E+01
-5.62E -5.62E
PENRM MJ 5.62E+01 0 0 0 0 0 0 0 0 0 0 0
+01 +01
PENRT MJ 2.18E+02 2.81E+00 6.68E+00 0 5.9E+00 0 1.56E-01 1.61E+00 2.32E+00 3.46E+00 -8.42E-01 0 -2.81E+01-5.06E+01
SM kg 6.03E-01 0 1.81E-02 0 0 0 0 0 0 0 0 0 0 6.3E-01
RSF MJ 0 0 0 0 0 0 0 0 0 0 0 0 0 0
NRSF MJ 0 0 0 0 0 0 0 0 0 0 0 0 0 0
FW m3 5.62E-02 1.8E-04 2.15E-03 0 3.34E-03 0 1E-05 1.53E-02 1.55E-02 4.05E-05 -2.2E-04 0 -7.32E-03 -4.58E-03
PERE = Use of renewable primary energy excluding renewable primary energy resources used as raw materials; PERM = Use of renewable primary
energy resources used as raw materials; PERT = Total use of renewable primary energy resources; PENRE = Use of non-renewable primary energy
excluding non-renewable primary energy resources used as raw materials; PENRM = Use of non-renewable primary energy resources used as raw
materials; PENRT = Total use of non-renewable primary energy resources; SM = Use of secondary material; RSF = Use of renewable secondary fuels;
NRSF = Use of non-renewable secondary fuels; FW = Use of net fresh water
5 Environmental Product Declaration - Fletco Carpets A/S - Woven carpet tiles, pile material PET, print design, maximum total pile weight 700 g/m², TEXtile backing
RESULTS OF THE LCA – WASTE CATEGORIES AND OUTPUT FLOWS according to EN 15804+A2:
1 m² floor covering
Parameter Unit A1-A3 A4 A5 B1 B2 C1 C2 C3/2 C3/3 C4/1 D D/1 D/2 D/3
HWD kg 4.55E-08 1.34E-11 1.37E-09 0 4.19E-05 0 7.47E-13 1.92E-10 2.22E-10 5.34E-10 -1.14E-10 0 -3.81E-09 -2.27E-10
NHWD kg 2.29E-01 4.02E-04 2.33E-02 0 7.3E-03 0 2.24E-05 5.46E-01 5.46E-01 3.43E+00 -4.24E-04 0 -1.41E-02 -1.05E-01
RWD kg 5.77E-03 3.45E-06 1.76E-04 0 3.76E-04 0 1.92E-07 8.1E-05 1.33E-04 4.25E-05 -6.59E-05 0 -2.2E-03 -1.05E-04
CRU kg 0 0 0 0 0 0 0 0 0 0 0 0 0 0
MFR kg 0 0 9.5E-02 0 0 0 0 0 6.3E-01 0 0 0 0 0
MER kg 0 0 0 0 0 0 0 0 0 0 0 0 0 0
EEE MJ 0 0 2.71E-01 0 0 0 0 9.02E+00 0 0 0 0 0 0
EET MJ 0 0 4.9E-01 0 0 0 0 1.63E+01 6.76E+01 0 0 0 0 0
HWD = Hazardous waste disposed; NHWD = Non-hazardous waste disposed; RWD = Radioactive waste disposed; CRU = Components for re-use;
MFR = Materials for recycling; MER = Materials for energy recovery; EEE = Exported electrical energy; EET = Exported thermal energy
RESULTS OF THE LCA – additional impact categories according to EN 15804+A2-optional:
1 m² floor covering
Parameter Unit A1-A3 A4 A5 B1 B2 C1 C2 C3/2 C3/3 C4/1 D D/1 D/2 D/3
Disease
PM 1.18E-07 7.2E-09 4.04E-09 0 6.84E-08 0 4.01E-10 8.73E-09 1.01E-08 6.94E-09 -5.38E-10 0 0 -2.39E-08
incidence
kBq U235
IR 9.54E-01 5.06E-04 2.9E-02 0 6.78E-02 0 2.82E-05 1.28E-02 2.15E-02 6.27E-03 -1.12E-02 0 0 -1.14E-02
eq
ETP-fw CTUe 8.9E+01 1.94E+00 2.76E+00 3.6E-03 2.69E+00 0 1.08E-01 9.04E-01 1.31E+00 3.39E+00 -1.84E-01 0 0 -8.85E+00
HTP-c CTUh 2.92E-09 3.93E-11 9.05E-11 0 6.21E-10 0 2.18E-12 5.36E-11 6.31E-11 1.52E-10 -8.48E-12 0 0 -9.8E-11
HTP-nc CTUh 1E-07 2.33E-09 3.16E-09 2.6E-11 9.46E-09 0 1.29E-10 2.92E-09 3.39E-09 1.27E-08 -3.26E-10 0 0 -5.68E-09
SQP SQP ND ND ND ND ND ND ND ND ND ND ND ND ND ND
PM = Potential incidence of disease due to PM emissions; IR = Potential Human exposure efficiency relative to U235; ETP-fw = Potential comparative
Toxic Unit for ecosystems; HTP-c = Potential comparative Toxic Unit for humans (cancerogenic); HTP-nc = Potential comparative Toxic Unit for humans
(not cancerogenic); SQP = Potential soil quality index
The SQP indicator is not given due to considerable uncertainties in the calculation.
The result figures given in module B2 refer to a period of 1 year because a reference service life is not declared. They have to be
multiplied by the assumed service life (in years) of the floor covering in the building under consideration.
Disclaimer 1 – for the indicator 'Potential Human exposure efficiency relative to U235'.
This impact category deals mainly with the eventual impact of low dose ionizing radiation on human health of the nuclear fuel cycle. It
does not consider effects due to possible nuclear accidents, occupational exposure or radioactive waste disposal in
undergroundfacilities. Potential ionizing radiation from the soil, radon and from some construction materials is also not measured by
this indicator.
Disclaimer 2 – for the indicators 'abiotic depletion potential for non-fossil resources', 'abiotic depletion potential for fossil resources',
'water (user) deprivation potential, deprivation-weighted water consumption', 'potential comparative toxic unit for ecosystems', 'potential
comparative toxic unit for humans – cancerogenic', 'Potential comparative toxic unit for humans - not cancerogenic', 'potential soil
quality index'.
The results of this environmental impact indicator shall be used with care as the uncertainties on these results are high as there is
limited experienced with the indicator.
References
EN 1307
DIN EN 1307: 2014+A1:2016+A2:2018-05: Textile floor ISO 10874
coverings - Classification DIN EN ISO 10874: 2012+A1:2021-04: Resilient, textile and
laminate floor coverings - Classification
EN 13501-1
DIN EN 13501-1:2019-05: Fire classification of construction ISO 14025
products and building elements - Part 1: Classification using DIN EN /ISO 14025:2011-10/, Environmental labels and
data from reaction to fire tests declarations — Type III environmental declarations —
Principles and procedures
EN 14041
DIN EN 14041: 2018-05 and DIN EN 14041: 2008-05: ISO 14040
Resilient, textile and laminate floor coverings - Essential DIN EN ISO 14040:2006+A1:2020 Environmental
characteristics management - Life cycle assessment - Principles and
framework
EN 15804
DIN EN 15804:2012+A2:2019 + AC:2021, Sustainability of ISO 14044
construction works — Environmental Product Declarations — DIN EN ISO 14044:2006+A1:2018+A2:2020 Environmental
Core rules for the product category of construction products management - Life cycle assessment - Requirements and
guidelines
EN 16810
DIN EN 16810: 2017-08: Resilient, textile and laminate floor ISO 15686
coverings – Environmental product declarations – Product ISO 15686: Buildings and constructed assets - Service life
category rules planning
6 Environmental Product Declaration - Fletco Carpets A/S - Woven carpet tiles, pile material PET, print design, maximum total pile weight 700 g/m², TEXtile backing
ISO 15686-1: 2011-05: Part 1: General principles and
framework GaBi database
ISO 15686-2: 2012-05: Part 2: Service life prediction GaBi Software-System and Database for Life Cycle
procedures Engineering, thinkstep AG, Leinfelden-Echterdingen, 2022-2
ISO 15686-7: 2017-04: Part 7: Performance evaluation for
feedback of service life data from practice PCR Part A
ISO 15686-8: 2008-06: Part 8: Reference service life and Product Category Rules for Building-Related Products and
service- Services Part A: Calculation Rules for the Life Cycle
life estimation Assessment and Requirements on the Project Report according
to EN 15804+A2:2019, V1.3, Berlin: Institut Bauen und Umwelt
Regulation (EU) No. 305/2011 e.V. (IBU), August 2022
Regulation No. 305/2011 Construction Products Regulation
(CPR) of the European Council and of the European PCR Part B
Parliament, April 2011 Product Category Rules for Building-Related Products and
Services Part B: Requirements on the EPD for floor coverings,
General Instructions for the IBU-EPD Program V1.3, Berlin: Institut Bauen und Umwelt e.V. (IBU), September
General Instructions for the EPD-Program of the Institut Bauen 2022
und Umwelt e.V., The Preparation of Environmental Product
Declarations - EPDs, version 2.0, Institut Bauen und Umwelt PRODIS
e.V., Berlin, January 2021, www.ibu-epd.de Product Information System (PRODIS) of the European Carpet
Industry, Gemeinschaft umweltfreundlicher Teppichboden e.V
BBSR (GUT) and European Carpet and Rug Association (ECRA),
Bundesinstitut für Bau-, Stadt- und Raumforschung (BBSR) im http://www.pro-dis.info
Bundesamt für Bauwesen und Raumordnung (BBR), Bonn
REACH
BNB, Nutzungsdauer von Bauteilen Regulation (EC) No 1907/2006 of the European Parliament and
Bewertungssystem Nachhaltiges Bauen (BNB), Nutzungsdauer of the Council of 18 December 2006 concerning the
von Bauteilen, Bundesministerium des Inneren, für Bau und Registration, Evaluation, Authorisation and Restriction of
Heimat, 24.02.2017 Chemicals (REACH), June 2017
ECHA candidate list VDZ e.V.
Candidate List of substances of very high concern (SVHCs) for Association of German Cement Works, Ed. Environmental Data
authorisation, last update 26.07.2022, European Chemicals of the German Cement Industry 2020
Agency (ECHA), Helsinki, Finland
7 Environmental Product Declaration - Fletco Carpets A/S - Woven carpet tiles, pile material PET, print design, maximum total pile weight 700 g/m², TEXtile backing
Publisher
Institut Bauen und Umwelt e.V. +49 (0)30 3087748- 0
Hegelplatz 1 info@ibu-epd.com
10117 Berlin www.ibu-epd.com
Germany
Programme holder
Institut Bauen und Umwelt e.V. +49 (0)30 3087748- 0
Hegelplatz 1 info@ibu-epd.com
10117 Berlin www.ibu-epd.com
Germany
Author of the Life Cycle Assessment
Gemeinschaft umweltfreundlicher Teppichboden +49 (0)241 96843 410
(GUT) e.V. mail@gut-ev.de
Schönebergstraße 2 www.gut-ev.org
52068 Aachen
Germany
Owner of the Declaration
Fletco Carpets A/S +45 (0)96 60 30 00
Mads Clausens Vej 2 fletco@fletco.dk
7441 Bording www.fletcocarpets.com
Denmark
8 Environmental Product Declaration - Fletco Carpets A/S - Woven carpet tiles, pile material PET, print design, maximum total pile weight 700 g/m², TEXtile backing
