ENVIRONMENTAL PRODUCT DECLARATION
as per ISO 14025 and EN 15804+A2
Owner of the Declaration Grundfos Holding A/S
Publisher Institut Bauen und Umwelt e.V. (IBU)
Programme holder Institut Bauen und Umwelt e.V. (IBU)
Declaration number EPD-GRU-20230078-CBC1-EN
Issue date 21.11.2023
Valid to 20.11.2028
MAGNA3 65-40/60 (Cast Iron)
Grundfos Holding A/S
www.ibu-epd.com | https://epd-online.com
General Information
Grundfos Holding A/S MAGNA3 65-40/60 (Cast Iron)
Programme holder Owner of the declaration
IBU – Institut Bauen und Umwelt e.V. Grundfos Holding A/S
Hegelplatz 1 Poul Due Jensens Vej 7
10117 Berlin 8850 Bjerringbro
Germany Denmark
Declaration number Declared product / declared unit
EPD-GRU-20230078-CBC1-EN Name of declared product / declared unit
This declaration is based on the product category rules: Scope:
Pumps for liquids and liquids with solids, 01.08.2021 The declaration applies to 1 piece of MAGNA3 (Cast Iron) pump.
(PCR checked and approved by the SVR)
The product is produced in Wahlstedt, Germany, and the life cycle
assessment is based on data collected at the production site.
Issue date
Production has been modeled using annual production data from 2021.
21.11.2023
The declaration covers two different types of the MAGNA3 65- product
(40/60).
Valid to
20.11.2028 The owner of the declaration shall be liable for the underlying information
and evidence; the IBU shall not be liable with respect to manufacturer
information, life cycle assessment data and evidences.
The EPD was created according to the specifications of EN 15804+A2. In
the following, the standard will be simplified as EN 15804.
Verification
The standard EN 15804 serves as the core PCR
Independent verification of the declaration and data according to ISO
14025:2011
Dipl.-Ing. Hans Peters internally X externally
(Chairman of Institut Bauen und Umwelt e.V.)
Florian Pronold Mrs Kim Allbury,
(Managing Director Institut Bauen und Umwelt e.V.) (Independent verifier)
1 Environmental Product Declaration - Grundfos Holding A/S - MAGNA3 65-40/60 (Cast Iron)
Product
Product description/Product definition Standards used:
The Grundfos MAGNA3 circulator pumps are designed for EN 60335-1:2012/AC:2014 + A11:2014, EN 60335-2-51:2003 +
circulating liquids in heating systems, air conditioning and A1:2008 + A2:2012,
cooling systems and domestic hot water systems. However, the EN 62233:2008.
pump range can also be used in ground source heat pump
systems and solar heating systems.
EN 55014-1:2006
+ A1:2009 + A2:2011, EN 55014-1:2017, EN 61000-6-2:2005,
The MAGNA3 pump is a centrifugal pump powered by an EN 61000-3-2:2014, EN
electrical motor. It has a high-performance neodymium magnet 61000-3-3:2013, ETSI EN 301 489-1 V2.2.0, ETSI EN 301 489-
rotor which increases motor efficiency and an insulation shell to 17 V3.2.0. ETSI EN
reduce heat loss from the cast iron pump housing with threaded 300 328 V2.1.1
connections.
The declaration covers two types of the MAGNA3 pump. They
are grouped as shown below. The group reference in the
technical data and scenarios refers also to these.
Electromagnetic
Compatibility (EMC) Directive (2014/30/EU)
GROUP 1 - MAGNA3 65-40
GROUP 2 - MAGNA3 65-60 Standards used:
EN 55014-1:2017, EN 55014-2:2015,
These are all the same physical products and 100 % identical
in terms of design, dimensions and materials as well as supply
chain and manufacturing processes, i.e., all cradle to gate
processes (A1-A3). EN
61000-3-2:2014/2019, EN 61000-6-2:2008/2019,
The products are also identical in terms of packaging,
distribution, reference service life and end-of-life treatment.
The only thing that differentiates the products from each other EN
is the software which controls how the pump operates in the 61000-3-3:2013 A1:2019
system in which it is installed, making them fit for different
applications. Hence, all life cycle modules are identical, except
use stage module B6, which will change, as the applied
scenarios for electricity consumption changes. For the placing
on the market in the European Union/European Free Trade
Association (EU/EFTA) (with the exception of Switzerland) the
following
legal provisions apply: RoHS Directive
2011/65/EU and 2015/863//EU
Machinery
Directive (2006/42/EC) Standard: EN
50581:2012.
Standard used: EN
809:1998 + A1:2009.
Ecodesign
Directive (2009/125/EC)
Radio Equipment
Directive (2014/53/EU) Commission
Regulation (EC) No: 641/2009 and
2 Environmental Product Declaration - Grundfos Holding A/S - MAGNA3 65-40/60 (Cast Iron)
Name Value Unit
Frequency 50 Hz
Commission
Voltage 230 V
Regulation (EU) 622/2012
Clean
Pumped liquid (e.g. water) -
Water
Energy Efficiency Index Gr.1 0,18
Standards used: Energy Efficiency Index Gr.2 0,17
EN 16297-1:2012, EN 16297-2:2012, EN 16297-3:2012. Flow range Gr. 1 (max) 23,0 m3/h
Flow range Gr. 2 (max) 32,0 m3/h
Head max. Gr.1 4 m
Head max. Gr. 2 6 m
Power input Gr. 1 Average (from load profile
0,109 m
describing use)
Power input Gr. 2 Average (from load profile
The CE marking takes into account the proof of conformity with 0,155 m
describing use)
the respective harmonized norms based on the legal provisions
Nominal capacity Gr.1 0,19 kW
above.
Nominal capacity Gr.2 0,342 kW
Performance data of the product according to the
harmonized standards, based on provisions for
MAGNA3 pumps harmonization.
are not harmonized in accordance with the CPR.
Base materials/Ancillary materials
Application
Base materials / Ancillary materials
For the application and use the respective national
Name Value Unit
provisions apply. Aluminium 13 %
Cast iron 54 %
Ceramics 0,3 %
Copper 3 %
The pump is designed for circulating liquids in the
Electronics 0,2 %
following systems: Magnet Nd 1 %
Paper 0,5 %
· heating systems
PCB 4 %
Plastics 0,3 %
· domestic hot-water systems
Plastics, foam 1 %
· air-conditioning and cooling systems Plastics GF 5 %
Rubber 0,2 %
· ground-source heat-pump systems
Stainless steel 4 %
Steel 5 %
· solar-heating systems
Cardboard 8 %
The pump is suitable for thin, clean, non-aggressive and non- Plastic film 0,1 %
explosive liquids, not containing solid particles or fibres that TOTAL 100 %
may attack the pump mechanically or chemically. In heating
REACH
systems, the water must meet the requirements of accepted
standards on water quality in heating systems. The pumps are
also suitable for domestic hot-water systems.
Technical Data
The performance data of the product according to the
harmonised norms, based on the harmonisation
provisions above apply.
This product/article/at
The relevant technical specifications according to the
least one partial article contains
PCR Part B are given in the table below. Characteristics
that are the same for all two product groups are
only given once. Others are given individually for all groups.
Constructional data
substances
listed in the ECHA candidate list (date:
10.06.2022)
exceeding 0.1 percentage by mass: no
3 Environmental Product Declaration - Grundfos Holding A/S - MAGNA3 65-40/60 (Cast Iron)
many factors, including many being scrapped prematurely
when e.g. the
boiler they are connected to is replaced.
The Wahlstedt
production has been assessed and certified as meeting the
requirements in ISO 14001,
ISO 50001, ISO 45001 and ISO 9001.
From the
estimated stock (140Mpa) and annual sales (14Mpa), the
average lifetime of
the circulator is taken as 10 years for the purposes of this study.
Reference service life
No use stage
scenario which refers to the lifetime of the product is declared.
However, to
facilitate building calculations, an estimated RSL of 10 years
can be used.
This is an EU consensus-based estimation, referenced on page The RSL of the
37 in Appendix 7: Lot declared product is not directly influencing the results in this
11 – Circulators in Buildings, prepared by AEA Energy & study, as no
Environment for declared use stage scenario is dependent on the RSL; The use
the European Commission in the context of the Eco Design stage sub-module
Directive: B6 is declared per year as required by the PCR Part B.
There is no
definitive information on the average circulator life available,
there is consensus
within the industry that it is at least 12 years. However, this is
complicated by
LCA: Calculation rules
20170712-n of
Declared Unit the SVR, the modules B3, B4 and B5 are by default declared
The declared as
unit is 1 piece (pcs.) of MAGNA3 (Cast Iron) pump. "MNR" (module not relevant).
Declared unit
Name Value Unit
Declared unit 1 pce.
Mass reference 23.17 kg/pce
Conversion factor [Mass/Declared Unit] 23.17
For IBU core EPDs (where clause 3.6 is part of the EPD): for
The product
average EPDs, an estimate of the robustness of the LCA
stage (A1-A3) comprises raw
values must be made, e.g. concerning the variability of the
material extraction and processing, transport processes as well
production process, geographical representativeness and the
as the
influence of background data and preliminary products
manufacturing process. The final production and assembly of
compared to the environmental impacts caused by the actual
the MAGNA3 pump
production.
takes place at a Grundfos manufacturing site in Germany.
However, the full
System boundary supply-chain leading to the finished product at the gate is rather
complex and
This EPD is
includes a large amount of raw materials, components and
Cradle-To-Grave. The system boundaries
semi-finished parts
which comes from both external suppliers as well as other
Grundfos production
facilities.
of the EPD
follow the modular approach in EN 15804. By decision no.
4 Environmental Product Declaration - Grundfos Holding A/S - MAGNA3 65-40/60 (Cast Iron)
·
A3 Production of ancillary materials or pre products;
·
A3 Manufacturing of products and coproducts;
The product
stage is included in the study, and according to EN 15804 the
system
boundary with nature is set to include those processes that ·
provide the A3 Manufacturing of packaging;
material and energy inputs into the system and the following
manufacturing,
transport up to the factory gate as well as the processing any
waste arising ·
from those processes. A1-A3 processing up to the end-of-waste state or disposal of
final residues.
Wastes and
losses are included in the modules where they occur according For secondary
to the polluter material inputs, the system boundary to the previous system
pays principle and the modular approach of EN 15804. (providing the
secondary material) is set where outputs reach the end-of-
waste state. The
recycling of secondary material into new raw materials is
included in the
system boundary of this study. Waste
The
product includes: materials from
production processes that are recycled without any modification
of the material's
inherent characteristics are modelled as closed-loop within A1-
· A3. This is done
A1 Extraction and processing of raw materials; up to the input mass flow that was used during production.
·
A1 Reuse of products or materials from a previous product
system;
Waste for
incineration arising in the product stage is accounted for in the
· module where
A1 Processing of secondary materials; the waste is produced. The environmental loads from the
incineration process
are declared in the module where it occurs and the electricity
and heat which
· is produced from the incineration are considered as closed-loop
A1 Generation of electricity, steam and heat from primary within A1-A3, as
energy resources, described in PCR Part A, 5.5.1. The input of biogenic carbon
also including their extraction, refining and transport; from the
production of packaging material is inventoried in A3. As
required by PCR
Part A, the corresponding end-of-life module of the packaging
· material, A5, is also declared and the emissions of biogenic
A1 Energy recovery and other recovery processes from carbon are
secondary fuels; inventoried.
·
A2 Transportation up to the factory gate and internal transport;
5 Environmental Product Declaration - Grundfos Holding A/S - MAGNA3 65-40/60 (Cast Iron)
The
construction process stage (A4-A5) includes:
A4:
Use stage
(B1-B7):
·
Transportation from factory gate to distribution center:
·
Consumption of electricity, thermal energy and water at The use stage,
distribution center; related to the building fabric includes:
· ·
Transportation from distribution center to construction site; B1, use or application of the installed product;
· ·
Wastage during distribution. B2, maintenance.
A5: The use stage
related to the operation of the building
·
Installation process; includes:
· ·
Transport of packaging waste to treatment site; B6, operational energy use;
· ·
Waste treatment of packaging. B7, operational water use.
The packaging In this study,
material does not reach the end of waste state but is all use stage modules are assessed, though B1, B2 and B7 are
incinerated as waste. assessed to be
According to European statistics, the average R1 value of zero. By decision no. 20170712-n of the SVR, the modules B3,
incineration plants B4 and B5
is > 0.6. Therefore, it is assumed are by default declared as "MNR" (module
that packaging not relevant).
material is treated thermally in an incineration plant with R1 > The modules include the provision and transport of all
0.6. The materials, products and
loads from the combustion process of packaging are declared related energy and water use, as well as waste processing up
in module A5 and to the
the resulting energy benefits in module end-of-waste state or disposal of final residues during the use
stage. They
also include all impacts and
D, as required
by the PCR Part A, 5.5.2.
6 Environmental Product Declaration - Grundfos Holding A/S - MAGNA3 65-40/60 (Cast Iron)
aspects related
to the losses during the use stage (i.e. production, transport,
and waste ·
processing and disposal of the lost products and materials). C1 deconstruction of the product from the
·
building, including initial on-site sorting of the
Generally, the
geographical coverage of the datasets used matches the actual ·
processes taking materials;
place. Meaning, that when modelling taking place in Grundfos
Bjerringbro,
the Danish electricity grid mix is used in the model and thermal
energy ·
from natural gas. These are generally of very high quality with C2 transportation of the discarded product to a recycling site
very good and
technological, temporal and geographical representativeness. transportation of waste to final disposal;
·
C3 waste processing, collection of waste fractions from the
deconstruction and
waste processing of material flows intended for reuse, recycling
Contributions and energy
to operational energy use during the use stage (B6) come from recovery;
the electricity
consumption of the product. The annual electricity consumption
is calculated by
multiplying the average power input, which is based on a ·
defined load profile, C4 waste disposal including physical pretreatment and
with the annual running hours. For use stage (B6) European management of the
Average disposal site.
electricity grid mix has been used. These values are declared in
the scenarios
section.
At the end of life,
the MAGNA3 pump is manually disassembled from the piping
system in which it has
been installed. The definition of the applied end-of-life scenario
in this EPD
follows the requirements in the
The End-of-Life
stage (C1-C4) includes all
activities from when the product reaches the end of its service PCR Part A, 6.2 regarding complex products, with a
life and no combination
longer provides any functionality and until all materials and of recycling, thermal waste treatment and landfilling. 100 % of
components are the material is
processed for considered in the end of life scenario as required by the PCR.
An
overall collection rate of 90 % has been assumed.
reuse/recycling
or disposed of.
Materials from
which energy is recovered in an incineration process with an
R1-value above 0.60
According to EN are in this study included with the environmental burdens from
15804 and the PCR Part A, the end-of-life stage the incineration
includes: process inventoried in C3, the recovered energy is declared as
exported energy
7 Environmental Product Declaration - Grundfos Holding A/S - MAGNA3 65-40/60 (Cast Iron)
in C3
and the energy
benefits are declared in D. This procedure is according to the
PCR Part A, Contributions
5.5.6. C3 includes the mechanical separation of the product to module D comes from waste incineration processes in A5
followed by a and C3 as well as
series of sorting steps. Metal fractions are recycled and material recycling in C3. The specific fractions and net flows are
plastics, cardboard shown in the
and electronics are assumed incinerated with energy recovery. scenarios section.
The residual
fractions are landfilled and declared in C4. Geographic Representativeness
Land or region, in which the declared product system is
manufactured, used or handled at the end of the product´s
lifespan: Europe
The specific
amounts are shown in the scenarios section.
Comparability
Basically, a comparison or an evaluation of EPD data is only
possible if all the data sets to be compared were created
according to EN 15804 and the building context, respectively
the product-specific characteristics of performance, are taken
into account. Software and databases used: GaBi ts
Beyond system
boundary (D): According to EN
15804 module D includes the reuse, recovery and/or recycling
potentials,
expressed as net impacts and benefits. Any declared benefits
and loads from net
9.2.1.68
(database schema 8007) Ecoinvent v3.5..
flows leaving
the product system that have not been allocated as co-products
and that have
passed the end-of-waste state are included in module D.
LCA: Scenarios and additional technical information
The following technical scenario information is required for the
Characteristic product properties of biogenic carbon declared modules and optional for non-declared modules.
The biogenic Modules for which no information is declared can be deleted;
carbon content quantifies the amount of biogenic carbon in a additional information can also be listed if necessary.
construction
product leaving the factory gate, and it will be separately The following technical information is a basis for the declared
declared for the modules or can be used for developing specific scenarios in the
product and for any accompanying packaging, as required from context of a building assessment if modules are not declared
the PCR Part A. (MND).
The Carbon content of Cardboard and Paper is assumed to
0.46 kg C. Overall, A5 is not declared including the disposal of the packaging
there is an amount of 9 weight-% Carbon in the product leaving material on the construction site, the amounts of packaging
the factory gate materials included in the LCA calculations must be declared as
and has to be considered technical scenario information for Module A5.
Transport from the gate to the site (A4)
Name Value Unit
Information on describing the biogenic Carbon Content at
Litres of fuel 0,0332 l/100km
factory gate
Transport distance 2003 km
Name ValueUnit
Capacity utilisation (including empty runs) 85 %
Biogenic carbon content in accompanying kg
0.74 Gross density of products transported 445 kg/m3
packaging C
Wastage during distribution 0,02 %
Note: 1 kg of biogenic carbon is equivalent to 44/12 kg of CO2
Installation into the building (A5)
8 Environmental Product Declaration - Grundfos Holding A/S - MAGNA3 65-40/60 (Cast Iron)
Name ValueUnit Name Value Unit
Packaging waste for incineration (LDPE film) 0,031 kg Collected as mixed construction waste 21,23 kg
Packaging waste for incineration Transportation distance (C2) 500 km
1,95 kg
(Paper/Cardboard) Aluminium for recycling 2,79 kg
An Steel for recycling 12,1 kg
estimated RSL of 10 years can be used to facilitate building Copper for recycling 0,51 kg
calculations. This
Stainless steel for recycling 0,84 kg
is an EU consensus-based estimation, referenced in Appendix
Plastics for incineration w/energy 1,38 kg
7: Lot 11 –
Electronics for incineration w/energy 0,81 kg
Circulators in Buildings, prepared by AEA Energy &
Environment for the Landfilling 2,8 kg
European Commission in the context of the Eco Design
Reuse, recovery and/or recycling potentials (D), relevant
Directive.
scenario information
Reference service life
Name Value Unit
Name Value Unit
A5, incineration w/energy recov. (LDPE foil) 4,37 MJ
Life Span according to the manufacturer 10 a
A5, incineration w/energy recov.
7,91 MJ
Operational energy use (B6) (Paper/Cardboard)
C3, steel for recycling (net amounts) -1,72 kg
Name Value Unit
C3, stainless steel for recycling (net amounts) 0,52 kg
Electricity consumption Group 1 545 kWh/a
C3, aluminium for recycling (net amounts) -0,383 kg
Electricity consumption Group 2 775 kWh/a
C3, copper for recycling (net amounts) 0,221 kg
Average power input, Group 1 0,109 kW
C3, plastics for incineration, w/ energy recov. 1,38 kg
Average power input, Group 2 0,155 kW
C3, electronics for incineration, w/ energy recov. 0,81 kg
Running hours (all groups) 5.000 h/a
End of life (C1-C4)
9 Environmental Product Declaration - Grundfos Holding A/S - MAGNA3 65-40/60 (Cast Iron)
LCA: Results
Characterization
model: EN 15804 - 2012+A2 - 2019, PEF. By Decision no. 20170712-n of the
IBU SVR, the modules B3, B4, B5 are marked as MNR (module not relevant) as
default. The LCA results in module B6 are given on a period of one year,
according to PCR Part B. To obtain the results from module B6 over the
entire life cycle, the LCA results of module B6 must be multiplied by the
estimated RSL of 10 years. The indicator results for module B6 are
declared for Group 1. B6 indicator results for other groups can be derived by
multiplying the B6 indicator results with the following factors:
Group 2: 1,422
DESCRIPTION OF THE SYSTEM BOUNDARY (X = INCLUDED IN LCA; ND = MODULE OR INDICATOR NOT DECLARED; MNR =
MODULE NOT RELEVANT)
Benefits and
Construction loads beyond
Product stage Use stage End of life stage
process stage the system
boundaries
la ire ta m w a Ry lp p u s tro p s n a rT g n iru tc a fu n a M e h t m o rf tro p s n a rTe tis e h t o t e ta g y lb m e s s A e s U e c n a n e tn ia M ria p e R tn e m e c a lp e R tn e m h s ib ru fe R y g re n e la n o ita re p Oe s u re ta w la n o ita re p Oe s u n o itc u rts n o c -e Dn o itilo m e d tro p s n a rT g n is s e c o rp e ts a W la s o p s iD -e s u e R-y re v o c e R-g n ilc y c e Rla itn e to p
A1 A2 A3 A4 A5 B1 B2 B3 B4 B5 B6 B7 C1 C2 C3 C4 D
X X X X X MND MND MNR MNR MNR X MND X X X X X
RESULTS OF THE LCA - ENVIRONMENTAL IMPACT according to EN 15804+A2: 1PCS of MAGNA3 65-40/60 (Cast Iron)
Parameter Unit A1 A2 A3 A4 A5 B6 C1 C2 C3 C4 D
GWP-total kg CO 2 eq 1.05E+02 1.41E+00 8.1E-01 1.45E+00 2.86E+00 2.2E+02 0 5.9E-01 6.57E+00 1.39E-01 4.59E-01
GWP-fossil kg CO 2 eq 1.05E+02 1.4E+00 4.05E+00 1.44E+00 1.53E-01 2.19E+02 0 5.87E-01 6.56E+00 1.43E-01 4.65E-01
GWP-
biogenic kg CO 2 eq 4.64E-01 -1.9E-03 -3.28E+00 -2.94E-03 2.7E+00 7.31E-01 0 -9.89E-04 6.35E-03 -4.3E-03 -3.62E-03
GWP-luluc kg CO 2 eq 1.8E-01 1.01E-02 3.66E-02 1.14E-02 9.69E-05 3.18E-01 0 4.77E-03 3.16E-03 1.25E-04 -2.74E-03
kg CFC11
ODP 9.52E-08 2.45E-16 4.07E-09 1.99E-11 5.23E-16 4.83E-12 0 1.08E-16 4.76E-14 3.21E-16 -7.63E-13
eq
AP mol H+ eq 5.54E-01 1.07E-02 1.7E-02 8.38E-03 8.22E-04 4.84E-01 0 3.47E-03 5.5E-03 4.43E-04 -9.34E-03
EP-
kg P eq 1.63E-03 3.85E-06 6.44E-05 4.63E-06 1.2E-07 5.86E-04 0 1.8E-06 8.37E-06 1.56E-05 -4.24E-06
freshwater
EP-marine kg N eq 7.15E-02 3.71E-03 3.3E-03 4E-03 3E-04 1.08E-01 0 1.67E-03 1.33E-03 1.02E-04 -1.03E-05
EP-terrestrial mol N eq 7.51E-01 4.11E-02 3.3E-02 4.43E-02 3.73E-03 1.13E+00 0 1.85E-02 1.49E-02 1.12E-03 3.31E-04
kg NMVOC
POCP 2.22E-01 8.55E-03 9.46E-03 7.61E-03 7.83E-04 2.95E-01 0 3.17E-03 3.64E-03 3.29E-04 -1.65E-05
eq
ADPE kg Sb eq 5.58E-03 1.05E-07 5.96E-05 1.24E-06 8.71E-09 6.35E-05 0 4.77E-08 6.27E-07 9.65E-09 -6.17E-04
ADPF MJ 1.43E+03 1.86E+01 5.62E+01 1.94E+01 9.85E-01 3.86E+03 0 7.86E+00 3.88E+01 2.05E+00 -1.44E+01
m3 world eq
WDP 2.59E+01 1.25E-02 2.36E-01 2.02E-02 3.52E-01 4.78E+01 0 5.75E-03 9.18E-01 -1.58E-03 -4.25E-01
deprived
GWP = Global warming potential; ODP = Depletion potential of the stratospheric ozone layer; AP = Acidification potential of land and water; EP =
Eutrophication potential; POCP = Formation potential of tropospheric ozone photochemical oxidants; ADPE = Abiotic depletion potential for non-fossil
resources; ADPF = Abiotic depletion potential for fossil resources; WDP = Water (user) deprivation potential)
RESULTS OF THE LCA - INDICATORS TO DESCRIBE RESOURCE USE according to EN 15804+A2: 1PCS of MAGNA3 65-40/60
(Cast Iron)
Parameter Unit A1 A2 A3 A4 A5 B6 C1 C2 C3 C4 D
PERE MJ 3.97E+02 9.73E-01 5.11E+01 1.21E+00 1.7E-01 1.71E+03 0 4.55E-01 1.68E+01 1.44E-01 3.69E+00
PERM MJ 0 0 0 0 0 0 0 0 0 0 0
PERT MJ 3.97E+02 9.73E-01 5.11E+01 1.21E+00 1.7E-01 1.71E+03 0 4.55E-01 1.68E+01 1.44E-01 3.69E+00
PENRE MJ 1.43E+03 1.87E+01 5.62E+01 1.94E+01 9.86E-01 3.86E+03 0 7.89E+00 3.88E+01 2.05E+00 -1.41E+01
PENRM MJ 0 0 0 0 0 0 0 0 0 0 0
PENRT MJ 1.43E+03 1.87E+01 5.62E+01 1.94E+01 9.86E-01 3.86E+03 0 7.89E+00 3.88E+01 2.05E+00 -1.41E+01
SM kg 1.79E+01 0 2.31E-01 3.62E-03 0 0 0 0 0 0 0
RSF MJ 1.46E-23 0 0 2.91E-27 0 0 0 0 0 0 0
10 Environmental Product Declaration - Grundfos Holding A/S - MAGNA3 65-40/60 (Cast Iron)
NRSF MJ 1.71E-22 0 0 3.42E-26 0 0 0 0 0 0 0
FW m3 8.11E-01 1.14E-03 2.57E-02 1.48E-03 8.29E-03 1.98E+00 0 5.3E-04 2.99E-02 2.6E-05 2.57E-02
PERE = Use of renewable primary energy excluding renewable primary energy resources used as raw materials; PERM = Use of renewable primary
energy resources used as raw materials; PERT = Total use of renewable primary energy resources; PENRE = Use of non-renewable primary energy
excluding non-renewable primary energy resources used as raw materials; PENRM = Use of non-renewable primary energy resources used as raw
materials; PENRT = Total use of non-renewable primary energy resources; SM = Use of secondary material; RSF = Use of renewable secondary fuels;
NRSF = Use of non-renewable secondary fuels; FW = Use of net fresh water
RESULTS OF THE LCA – WASTE CATEGORIES AND OUTPUT FLOWS according to EN 15804+A2:
1PCS of MAGNA3 65-40/60 (Cast Iron)
Parameter Unit A1 A2 A3 A4 A5 B6 C1 C2 C3 C4 D
HWD kg 3.3E-04 7.76E-07 1.22E-04 9.59E-07 5.11E-09 1.6E-06 0 3.65E-07 1.96E-08 8.21E-09 -3.25E-04
NHWD kg 4.12E+00 2.85E-03 2.91E-01 4.09E-03 9.43E-02 2.74E+00 0 1.25E-03 6.3E-01 2.35E+00 2.35E+00
RWD kg 6.2E-02 3.3E-05 1.55E-03 5.25E-05 4.74E-05 5.85E-01 0 1.46E-05 5.75E-03 2.45E-05 -1.8E-03
CRU kg 0 0 0 0 0 0 0 0 0 0 0
MFR kg 0 0 0 0 0 0 0 0 1.63E+01 0 0
MER kg 0 0 0 0 0 0 0 0 0 0 0
EEE MJ 0 0 0 0 4.37E+00 0 0 0 7.4E+00 0 0
EET MJ 0 0 0 0 7.91E+00 0 0 0 1.33E+01 0 0
HWD = Hazardous waste disposed; NHWD = Non-hazardous waste disposed; RWD = Radioactive waste disposed; CRU = Components for re-use;
MFR = Materials for recycling; MER = Materials for energy recovery; EEE = Exported electrical energy; EET = Exported thermal energy
RESULTS OF THE LCA – additional impact categories according to EN 15804+A2-optional:
1PCS of MAGNA3 65-40/60 (Cast Iron)
Parameter Unit A1 A2 A3 A4 A5 B6 C1 C2 C3 C4 D
Disease
PM 6.83E-06 1.27E-07 2.37E-07 4.98E-08 4.65E-09 4.06E-06 0 2.03E-08 4.65E-08 4.52E-09 -2.53E-07
incidence
IR kBq U235 eq 6.81E+00 4.86E-03 2.44E-01 7.34E-03 7.3E-03 9.6E+01 0 2.15E-03 9.42E-01 3.48E-03 -1.54E-01
ETP-fw CTUe 8.38E+02 1.38E+01 1.82E+01 1.42E+01 4.97E-01 1.65E+03 0 5.88E+00 1.69E+01 1.44E+00 -5.41E+00
HTP-c CTUh 1.62E-06 2.84E-10 6.46E-07 7.48E-10 2.44E-11 4.56E-08 0 1.22E-10 5.13E-10 8.27E-11 -6.64E-08
HTP-nc CTUh 2.45E-06 1.55E-08 5.68E-08 1.72E-08 1.15E-09 1.68E-06 0 6.98E-09 2.07E-08 7.21E-09 4.97E-10
SQP SQP 4.09E+02 5.87E+00 9.71E+01 6.7E+00 2.68E-01 1.23E+03 0 2.76E+00 1.22E+01 1.48E-01 -1.61E+01
PM = Potential incidence of disease due to PM emissions; IR = Potential Human exposure efficiency relative to U235; ETP-fw = Potential comparative
Toxic Unit for ecosystems; HTP-c = Potential comparative Toxic Unit for humans (cancerogenic); HTP-nc = Potential comparative Toxic Unit for humans
(not cancerogenic); SQP = Potential soil quality index
Disclaimer
1 – for the indicator 'Potential Human exposure efficiency relative to U235'.
This impact category deals mainly with the eventual impact of low-dose ionizing
radiation on human health of the nuclear fuel cycle. It does not consider
effects due to possible nuclear accidents, occupational exposure or
radioactive waste disposal in underground facilities. Potential ionizing
radiation from the soil, radon and from some construction materials is
also not measured by this indicator.
Disclaimer 2 – for the
indicators 'abiotic depletion potential for non-fossil resources', 'abiotic
depletion potential for fossil resources', 'water (user) deprivation potential,
deprivation-weighted water consumption', 'potential comparative toxic unit for
ecosystems', 'potential comparative toxic unit for humans – cancerogenic',
'Potential comparative toxic unit for humans - not cancerogenic', 'potential
soil quality index'. The results of this environmental impact indicator shall
be used with care as the uncertainties on these results are high as there is
limited experience with the indicator.
Disclaimer 3: JRC
Technical Reports, Version 2, 2018 Page 6, for the
indicator "EP-freshwater". This indicator has been calculated as 'kg
P eq' as required in the characterization model EUTREND model, Struijs et al.,
11 Environmental Product Declaration - Grundfos Holding A/S - MAGNA3 65-40/60 (Cast Iron)
2009b, as implemented in ReCiPe; This EPD was created using a software tool.
References
Standards
2014 on the
harmonistion of the laws of the Member
Machinery States relating
Directive to electromagnetic compatibility
DIRECTIVE 2006/42/EC
OF THE EUROPEAN
Ecodesign
PARLIAMENT AND Directive
OF THE COUNCIL of 17 May
DIRECTIVE
2006 on 2009/125/EC OF THE EUROPEAN
machinery
PARLIAMENT AND
OF THE COUNCIL of 21 October
Radio Equipment 2009
Directive establishing a framework for the setting of
DIRECTIVE ecodesign
2014/53/EU OF THE EUROPEAN PARLIAMENT AND OF THE requirements for energy-related products
COUNCIL of 16 April 2014 on
the harmonisation of the laws of the Member States relating to
the making
available on the market of
radio equipment EC 641/2009
COMMISSION
REGULATION (EC) No 641/2009 of 22 July 2009 implementing
Directive 2005/32/EC
of the European Parliament and of the Council with regard to
Electromagnetic ecodesign
Compatibility (EMC) Directive requirements for glandless standalone circulators and
glandless circulators integrated
in
DIRECTIVE
2014/30/EU OF THE EUROPEAN
products
PARLIAMENT AND
OF THE COUNCIL of 26 February
12 Environmental Product Declaration - Grundfos Holding A/S - MAGNA3 65-40/60 (Cast Iron)
substances
EC 622/2012
COMMISSION
REGULATION (EU) No 622/2012 of 11 July 2012 amending ETSI EN 301
Regulation (EC) No 489-1
641/2009 with regard to ecodesign requirements for glandless
standalone
circulators and glandless circulators integrated in products
ETSI EN 301
489-1 V2.2.0, Electromagnetic Compatibility (EMC) standard for
radio equipment
and services; Part 1: Common technical requirements
DIRECTIVE
2011/65/EU
ETSI EN 301
DIRECTIVE 489-17
2011/65/EU OF THE EUROPEAN
ETSI EN 301
PARLIAMENT AND 489-17 V3.2.0, Electromagnetic Compatibility (EMC) standard
OF THE COUNCIL of 8 June 2011 for radio equipment
and services; Part 17: Specific conditions for Broadband Data
Transmission
Systems
on the
restriction of the use of certain hazardous
substances in
electrical and electronic equipment
DIRECTIVE
2015/863/EU ETSI EN 300 328
V2.1.1
DIRECTIVE
2015/863/EU of 31 March 2015 amending ETSI EN 300 328
V2.1.1, Wideband transmission systems; Data transmission
equipment operating in
the 2,4 GHz ISM band and using wide band modulation
Annex II to techniques
Directive 2011/65/EU of the European
Parliament and
of the Council as regards the list of
EN 809
restricted
13 Environmental Product Declaration - Grundfos Holding A/S - MAGNA3 65-40/60 (Cast Iron)
EN 809:1998-10
+ A1:2009, Pumps and pump units for
respect to the
restriction of hazardous substances
liquids -
Common safety requirements
EN 60335-1
EN 55014-1
EN
60335-1:2012/A11:2014/A13:2017, Household
EN
55014-1:2017, Electromagnetic compatibility – Requirements
for household and similar
appliances, electric tools and similar apparatus – Part 1: electrical appliances – Safety – Part 1:General requirements
Emission
EN 60335-2-51
EN 55014-2
EN
EN 60335-2-51:2003-03 + A1:2008 + A2:2012, Household and
55014-2:2015, Electromagnetic compatibility – similar electrical
appliances – Safety –Part 2-51: Particular requirements for
stationary
circulation pumps for heating and service water installations
Requirements
for household appliances, electric tools
and similar
apparatus – Part 2: Immunity – Product
EN 61000-3-2
family standard
(CISPR 14-2:2015) EN
61000-3-2:2014/2019, Electromagnetic compatibility (EMC) –
Part 3-2: Limits –
Limits for harmonic current emissions (equipment input current
=16 A per phase)
EN 50581:2012
EN 50581:2012, EN 61000-3-3
Technical documentation for the
EN
assessment of 61000-3-3:2013-08/ A1:2019, Electromagnetic compatibility
electrical and electronic products with (EMC) – Part 3-3:
14 Environmental Product Declaration - Grundfos Holding A/S - MAGNA3 65-40/60 (Cast Iron)
Limits – Limitation of voltage changes, voltage fluctuations and
flicker in public
low voltage supply systems, for equipment with
EN 16297-3
rated current
<= 16 A per phase and not subject to conditional connection
EN
16297-3:2012, Pumps – Rotodynamic pumps –Glandless
circulators – Part 3: Energy
efficiency index (EEI) for circulators integrated in products
EN 61000-6-2
EN ISO 14001
61000-6-2:2008/2019, Electromagnetic compatibility (EMC) –
Part 6-2: Generic
standards –Immunity for industrial environments
EN ISO
14001:2015-09, Environmental management systems -
Requirements with guidance
for use
EN 16297-1
EN ISO 14025
16297-1:2012-10, Pumps – Rotodynamic pumps –Glandless
circulators – Part 1:
General requirements and procedures for testing and
calculation of energy DIN EN /ISO
efficiency index (EEI) 14025:2011-10, Environmental labels and declarations — Type
III environmental
declarations — Principles and procedures
EN 15804
EN
15804:2012-04+A1 2013, Sustainability of construction works
— Environmental
Product Declarations — Core rules for the product category of
construction
products
EN 16297-2
EN 16297-2:2012-10,
Pumps – Rotodynamic pumps –Glandless circulators – Part 2:
Calculation of
energy efficiency index (EEI) for standalone circulators PCR Part A
15 Environmental Product Declaration - Grundfos Holding A/S - MAGNA3 65-40/60 (Cast Iron)
Institut Bauen
und Umwelt e.V., Berlin (pub.): Product Category Rules for
Building-Related
Products and Services, Product Category Rules for
Construction Products from
the range of Environmental Product Declarations of Institut
Bauen und Umwelt
(IBU), Part A: Calculation Rules for the Life Cycle Assessment CML 2001
and Requirements
on the Project Report, Version 1.7 (2021)
Impact
assessment characterization factors Institute of Environmental
Sciences, Leiden
University, Netherlands
PCR
Part B
Institut Bauen ECHA candidate
und Umwelt e.V., Berlin (pub.): Product Category Rules for list
Building-Related
Products and Services, Product Category Rules for
Construction Products from
the range of Environmental Product Declarations of Institut Candidate List
Bauen und Umwelt of substances of very high concern (SVHCs) for authorisation,
(IBU), Part B: Requirements on the EPD for Pumps for liquids European
and liquids with Chemicals Agency (ECHA), Helsinki, Finland
solids, Version 1.0 (2018)
Ecoinvent
Ecoinvent v3.5
GaBi ts
Further
references
GaBi ts 9.2.1.68
(database schema 8007)
CPR
REACH
REGULATION (EU)
No 305/2011 OF THE EUROPEAN PARLIAMENT AND OF
THE COUNCIL of 9 March 2011
laying down harmonised conditions for the marketing of Regulation (EC)
construction products No 1907/2006 of the European Parliament and of the Council of
and repealing Council Directive 89/106/EEC 18 December 2006
16 Environmental Product Declaration - Grundfos Holding A/S - MAGNA3 65-40/60 (Cast Iron)
concerning the Registration, Evaluation, Authorisation and Advisory Board
Restriction of (formerly SVA)
Chemicals (REACH) (Status: 27.06.2018)
Decision no.
20170712-n
The literature referred to in the Environmental Product
Declaration must be listed in full.Standards already fully quoted
SVR in the EPD do not need to be listed here again.
The current version of PCR Part A and PCR Part B of the PCR
document on which they are based must be referenced.
17 Environmental Product Declaration - Grundfos Holding A/S - MAGNA3 65-40/60 (Cast Iron)
Publisher
Institut Bauen und Umwelt e.V. +49 (0)30 3087748- 0
Hegelplatz 1 info@ibu-epd.com
10117 Berlin www.ibu-epd.com
Germany
Programme holder
Institut Bauen und Umwelt e.V. +49 (0)30 3087748- 0
Hegelplatz 1 info@ibu-epd.com
10117 Berlin www.ibu-epd.com
Germany
Author of the Life Cycle Assessment
Grundfos Holding A/S +45 87501400
Poul Due Jensens Vej 7 atomic@grundfos.com
8850 Bjerringbro www.grundfos.com
Denmark
Owner of the Declaration
Grundfos Holding A/S +45 87501400
Poul Due Jensens Vej 7 atomic@grundfos.com
8850 Bjerringbro www.grundfos.com
Denmark
18 Environmental Product Declaration - Grundfos Holding A/S - MAGNA3 65-40/60 (Cast Iron)
