ENVIRONMENTAL PRODUCT DECLARATION
as per ISO 14025 and EN 15804+A2
Owner of the Declaration fischerwerke GmbH & Co. KG
Publisher Institut Bauen und Umwelt e.V. (IBU)
Programme holder Institut Bauen und Umwelt e.V. (IBU)
Declaration number EPD-DBC-FIW-20230414-IBF1-EN
Issue date 20.11.2023
Valid to 07.06.2027
FiAM Plus
fischerwerke GmbH & Co. KG
www.ibu-epd.com | https://epd-online.com
1. General Information
fischerwerke GmbH & Co. KG FiAM Plus
Programme holder Owner of the declaration
IBU – Institut Bauen und Umwelt e.V. fischerwerke GmbH & Co. KG
Hegelplatz 1 Klaus­Fischer­Straße 1
10117 Berlin 72178 Waldachtal
Germany Germany
Declaration number Declared product / declared unit
EPD­DBC­FIW­20230414­IBF1­EN 1 kg / 1 kg; density 1,63 ­ 1,73 g/cm³
This declaration is based on the product category rules: Scope:
Dispersion adhesives and primers for floor coverings, 01.08.2021 This is a manufacturer­individualised EPD based on model declaration
(PCR checked and approved by the SVR) "Dispersion­based products, group 1" (EPD­DBC­20220146­IBF1­EN)
from Deutsche Bauchemie e.V. in which the product which exhibits the
highest environmental impact in a particular group was selected from the
Issue date group to calculate the LCA.
20.11.2023
This verified EPD entitles the holder to bear the symbol of the Institut
Bauen und Umwelt e.V. It exclusively applies to products produced in
Europe and applies to a period of five years from the date of issue. This
Valid to
EPD may be used by members of DBC, EFCC, FEICA and IVK and their
07.06.2027 members provided. It has been proven that the respective product can be
represented by this EPD.
The owner of the declaration shall be liable for the underlying information
and evidence; the IBU shall not be liable with respect to manufacturer
information, life cycle assessment data and evidences.
The EPD was created according to the specifications of EN 15804+A2. In
the following, the standard will be simplified as EN 15804.
Verification
The standard EN 15804 serves as the core PCR
Independent verification of the declaration and data according to ISO
Dipl.­Ing. Hans Peters
14025:2011
(Chairman of Institut Bauen und Umwelt e.V.)
internally X externally
Florian Pronold Matthias Schulz,
(Managing Director Institut Bauen und Umwelt e.V.) (Independent verifier)
1 Environmental Product Declaration ­ fischerwerke GmbH & Co. KG ­ FiAM Plus
2. Product
2.1 Product description/Product definition 2.5 Base materials/Ancillary materials
fischer FiAM Plus is a one part water­based acrylic sealant ­ Synthetic polymer dispersion (solids portion): 10 ­ 25
which has been designed to provide smoke and fire protection ­ Mineral fillers: 50 ­ 75
on construction joints and single penetrations in both vertical ­ Water: 5 ­ 15
and horizontal applications. It dries physically through the ­ Auxiliaries: 5 ­ 10
evaporation of the water contained therein. When exposed to ­ Thickening agents: < 3
fire, it reacts to form a highly insulative char that slows down ­ Dispersing agents/Emulsifying agents: < 2
heat transfer and provides a barrier to fire. Formulated to be ­ Other: 0 ­ 2
halogen and solvent free. FiAM Plus has been designed to
maintain the sound reduction index of a structure. ­ VOC according to Decopaint Directive: <1 % (mandatory)
The product displaying the highest environmental impacts This product contains substances listed in the candidate list
within the class of dispersion­based products considered was (date: 06.07.2023) exceeding 0.1percentage by mass: no
used as a representative product for calculating the Life Cycle
Assessment results (worst­case approach). For the placing of This product contains other carcinogenic, mutagenic, reprotoxic
the product on the market in the European Union European (CMR) substances in categories 1A or 1B which are not on the
Free Trade Association (EU/EFTA) (with the exception of candidatelist, exceeding 0.1 percentage by mass: no
Switzerland) Regulation (EU) No. 305/2011 (CPR) applies.
Biocide products were added to this construction product: yes
Hence, the product is CE­marked and requires a declaration of
performance based on the performance assessed in the This construction product contains biocides for in­can
European Technical Approvals ETA-23/0163 and ETA-23/0165. preservation. The product contains reaction mass of 5­chloro­2­
methyl­2H­isothiazol­3­one and 2­methyl­2H­isothiazol3­one
Furthermore, this product is certified by UL: Representative (3:1) and 1,2­benzisothiazol­3(2H)­one as active substances.
samples of this product have been evaluated by UL against Further information is listed in the safety data sheet of this
EN­, UL­ and ASTM standards. As a result, the production is product.
subject to regular audits and the product bares the UL­US and
UL­EU mark and is UL listed at UL product IQ, UL's global, 2.6 Manufacture
online product directory. All raw materials are sourced in Europe. The transport is
exclusively by truck. The product is mixed discontiously in batch
For the application and use of the products the respective mode and filled into the delivery containers. Process control
national provisions apply. technology is used to weigh and mix solid and liquid raw
materials according to the recipe. Documentation of the
2.2 Application production process is also done automatically by the process
fischer FiAM Plus is an acrylic­based sealant used to form a control system.
penetration seal around penetration elements such as pipes The manufacturing plant of FiAM Plus, fischerwerke GmbH &
and cables, to reinstate the fire resistance performance of wall Co. KG, Otto­Hahn­Str. 15, 79211 Denzlingen, Germany, is
and floor constructions where they have been provided with certified according to ISO 14001 which defines international
apertures for the penetration of services. It is also used to form standards for sustainable environmental management.
linear joint seals within wall and floor constructions.
fischer FiAM Plus is supplied in liquid form contained within 310 2.7 Environment and health during manufacturing
ml and 600 ml foils. The sealant is gunned or trowelled into the As a general rule, no particular environmental or health
aperture in or between the separating element/elements to a protection measures other than those specified by law are
specified depth using various backing materials. necessary.
2.3 Technical Data 2.8 Product processing/Installation
The density of the products is between 1,63 and 1,73 g/cm³, The sealant is gunned or trowelled into the aperture in or
other relevant technical data can be found in the manufacturer's between the separating element/elements to a specified depth
technical documentation. using various backing materials.
Precautions for safe handling and storage (e.g. personal
Constructional data
protective measures, conditions for safe storage) must be
Name Value Unit observed in accordance with the information on the safety data
Density (mean value) EN ISO 1183­1 1,68 g/ml sheet.
Additional technical data are not relevant for FiAM Plus.
The applied film thickness and width depends on the
application. The specifications from the certification documents
must be adhered to.
Performance data of the product in accordance with
the declaration of performance with respect to its essential
2.9 Packaging
characteristics according to ETA­23/0163 and ETA­23/0165 and
A detailed description of packaging is provided in section 2.4.
the different UL listings.
Empty cartridges can be recycled. The product can be disposed
2.4 Delivery status with household waste.
Sold in plastic cartridges of 310 ml or foil bags of 600 ml.
2.10 Condition of use
During the use phase, dispersion­based products are existent
A plastic container was modelled for the Life Cycle Assessment.
as hardened film. They are long­lasting products which protect
2 Environmental Product Declaration ­ fischerwerke GmbH & Co. KG ­ FiAM Plus
our buildings in the form of adhesives, primers, coatings or
sealants as well as make an essential contribution towards their Water
appearance, function and sustainability. Dispersion­based products are water­resistant only to a certain
degree and their strength can deteriorate when exposed to
2.11 Environment and health during use water for longer periods (of time); detaching from the surface is
No risks are known for water, air and soil if the products are possible in a worst­case scenario. The components of
used as designated. dispersion­based products are not hazardous to water or only
slightly hazardous to water. Owing to the overall low volumes of
2.12 Reference service life
dispersion­based products used on buildings, no relevant
The provisions made in the European Technical Assessment contribution towards environmental damage can be anticipated
are based on an assumed working life of FiAM Plus of 25 by buildings featuring dispersion­ based products in the event
years, provided that the conditions laid down in the product of extraordinary exposure to water.
datasheet for the packaging / transport / storage / installation /
use / repair are met. The indications given on the working life Mechanical destruction
cannot be interpreted as a guarantee given by the producer or The mechanical destruction of dispersion­based products does
the Technical Assessment Body, but are to be regarded only as not lead to any decomposition­products which are harmful to
a means for choosing the right products in relation to the the environment or health.
expected economically reasonable working life of the works.
Description of the influences on the ageing of the product when 2.14 Re­use phase
applied in accordance with the rules of technology. According to present knowledge, no environmentally hazardous
effects in terms of landfilling are to be generally anticipated
through dismantling and recycling components to which
2.13 Extraordinary effects
dispersion­based products have been applied and on which
Fire
they have dried.
The FiAM Plus (at cured state) complies with the requirements
of the DIN EN 13501-1 standard for fire class D­s1,d0. 2.15 Disposal
Additionally, the product is tested according to ASTM E84 / The product can be disposed with normal household waste.
UL723-11 as per International Building code 2021, section EAK Codes:
803.1.2: Flame spread index class A, Smoke development 20 00 00 MUNICIPAL WASTES (HOUSEHOLD WASTE AND
index: class A. SIMILAR COMMERCIAL, INDUSTRIAL AND INSTITUTIONAL
The product's resistance to fire is detailed in the certification WASTES) INCLUDING SEPARATELY COLLECTED
documents. FRACTIONS
Fire protection
or
Name Value
EN 13501­1
08 04 10 waste adhesives and sealants other than those
Building material class D mentioned in 08 04 09
Smoke gas development s1
2.16 Further information
Burning droplets d0
More information is available on www.fischer­international.com.
ASTM E84
Flame spread index class A
Smoke development index class A
3. LCA: Calculation rules
Modules A1, A2 and A3 are taken into consideration in the LCA:
3.1 Declared Unit
This EPD refers to the declared unit of 1 kg of dispersion­based
product, group 1; applied into the building with a density of ­ A1
1,000 ­ 1,500 kg/m³ in accordance with the IBU PCR part B for Production of preliminary products
dispersion adhesives and primers for floor coverings.
The results of the Life Cycle Assessment provided in this
declaration have been selected from the product with the ­ A2
highest environmental impact (worst­case scenario). Transport to the plant
Depending on the application, a corresponding conversion
factor such as the density to convert volumetric use to mass
must be taken into consideration. ­ A3
Production incl. provision of energy, production of packaging as
The Declaration type is according to EN 15804: Cradle to gate well as
with options, modules C1–C3, and module D (A1–A3, C, D) and auxiliaries and consumables and waste treatment
additional modules (A4­A5).
Declared unit
­ A4 Transport
Name Value Unit
to site
Declared unit 1 kg
Gross density 1,000­1,500 kg/m3
­ A5
3.2 System boundary Installation, product applied into the building during A5 phase
operations and
3 Environmental Product Declaration ­ fischerwerke GmbH & Co. KG ­ FiAM Plus
packaging disposal. required for the production of the products under review was
The end of life for the packaging material considered is not taken into consideration in the LCA.
described below:
Transport of packaging materials is excluded.
­ Incineration, for materials like plastic and wood.
3.5 Background data
Data from the GaBi database SP40 (2020) was used as
­ C1­C2­C3­D background data.
3.6 Data quality
The building deconstruction (demolition process) takes place in Representative products were applied for this EPD and the
the C1 module which considers energy production and product in the group displaying the highest environmental
consumption in terms of diesel and all the emissions connected impact was selected for calculating the LCA results. The
with the fuel­burning process to run the machines. After the background datasets used are less than 4 years old.
demolition, the product is transported to the end­of­life
processing (C2 module) where all the impacts related to the
transport processes are considered. For precautionary principle Production data and packaging are based on details provided
and as a worst­case scenario, thermal treatment is the only end by the manufacturer. The formulation used for evaluation refers
of life scenario considered. This is modelled by the incineration to a specific product.
process (module C3) where the product ends its life cycle.
The data quality of the background data is considered to be
Module D good.
accounts for potential benefits that are beyond the defined
3.7 Period under review
system boundaries.
Representative formulations are valid for 2021.
Credits are generated during the incineration of wastes and
related electricity 3.8 Geographic Representativeness
produced that are occurring in the A5 module.
Land or region, in which the declared product system is
3.3 Estimates and assumptions manufactured, used or handled at the end of the product´s
lifespan: Europe
For this EPD formulation and production data defined and
collected by FEICA were
considered. Production waste was assumed to be disposed of 3.9 Allocation
by incineration without credits as a worst­case.
Mass allocation has been applied when primary data have
been used and implemented into the LCA model.
An average of plastic containers and wooden pallets was
considered in the LCA. 3.10 Comparability
Basically, a comparison or an evaluation of EPD data is only
3.4 Cut­off criteria
possible if all the data sets to be compared were created
All raw materials submitted for the formulations and production
according to EN 15804 and the building context, respectively
data were taken into
the product­specific characteristics of performance, are taken
consideration.
into account. Data from the GaBi database SP40 (2020) was
used as background data.
The manufacture of machinery, plant and other infrastructure
4. LCA: Scenarios and additional technical information
Transport to the building site (A4)
Characteristic product properties of biogenic carbon
The packaging material contains biogenic carbon content which Name Value Unit
is presented below. Transport distance 1000 km
Information on describing the biogenic Carbon Content at Gross weight 34 ­ 40 t
factory gate Payload capacity 27 t
Name ValueUnit
Installation into the building (A5)
kg
Biogenic carbon content in product ­ Name Value Unit
C
Other resources for packaging material 0.067 kg
Biogenic carbon content in accompanying kg
packaging 0.016 C Material loss 0.01 kg
For the preparation of building life cycle assessments, it must Material loss regards the amount of product not used during the
be taken into account that in module A5 (installation in the application phase into the building. This amount is 1% of the
building) the biogenic amount of CO (0.016 kg C *3.67 = 0.059 product, impacts related to the production of this part are
2
charged to the A5 module. This percentage is considered as
kg CO ­eq.) of the packaging bound in module A1­A3 is
2 waste to disposal and impacts of its end of life have been
mathematically booked out.
considered in the LCA model and declared in A5.
Note: 1 kg of biogenic carbon is equivalent to 44/12 kg of CO2 End of life (C1­C3)
4 Environmental Product Declaration ­ fischerwerke GmbH & Co. KG ­ FiAM Plus
Name Value Unit
Collected as mixed construction waste 1 kg
Incineration 1 kg
5 Environmental Product Declaration ­ fischerwerke GmbH & Co. KG ­ FiAM Plus
5. LCA: Results
DESCRIPTION OF THE SYSTEM BOUNDARY (X = INCLUDED IN LCA; ND = MODULE OR INDICATOR NOT DECLARED; MNR =
MODULE NOT RELEVANT)
Benefits and
Construction loads beyond
Product stage Use stage End of life stage
process stage the system
boundaries
la ire ta m w a Ry lp p u s tro p s n a rT g n iru tc a fu n a M e h t m o rf tro p s n a rTe tis e h t o t e ta g y lb m e s s A e s U e c n a n e tn ia M ria p e R tn e m e c a lp e R tn e m h s ib ru fe R y g re n e la n o ita re p Oe s u re ta w la n o ita re p Oe s u n o itc u rts n o c ­e Dn o itilo m e d tro p s n a rT g n is s e c o rp e ts a W la s o p s iD ­e s u e R­y re v o c e R­g n ilc y c e Rla itn e to p
A1 A2 A3 A4 A5 B1 B2 B3 B4 B5 B6 B7 C1 C2 C3 C4 D
X X X X X MND MND MNR MNR MNR MND MND X X X MND X
RESULTS OF THE LCA ­ ENVIRONMENTAL IMPACT according to EN 15804+A2: 1 kg of dispersion­based product, group 1
Parameter Unit A1­A3 A4 A5 C1 C2 C3 D
GWP­total kg CO 2 eq 1.32E+00 5.11E­02 1.73E­01 2.79E­04 1.24E­02 9.45E­01 ­3.98E­01
GWP­fossil kg CO 2 eq 1.36E+00 5.06E­02 8.81E­02 2.66E­04 1.18E­02 4.29E­01 ­3.97E­01
GWP­biogenic kg CO 2 eq ­5.05E­02 1.48E­04 8.53E­02 1.24E­05 5.42E­04 5.15E­01 ­8.96E­04
GWP­luluc kg CO 2 eq 4.52E­04 4.1E­04 6.04E­06 6.39E­09 2.79E­07 3.5E­05 ­2.51E­04
ODP kg CFC11 eq 3E­14 6.08E­18 3.18E­16 2.84E­20 1.24E­18 3.02E­16 ­3.72E­15
AP mol H+ eq 4.9E­03 1.52E­04 7.29E­05 3.6E­06 3.73E­05 5.25E­04 ­5.26E­04
EP­freshwater kg P eq 2.65E­05 1.54E­07 2.68E­07 5.75E­11 2.51E­09 1.04E­07 ­4.62E­07
EP­marine kg N eq 1.03E­03 6.75E­05 1.75E­05 1.63E­06 1.72E­05 2.01E­04 ­1.39E­04
EP­terrestrial mol N eq 1.24E­02 7.56E­04 2.36E­04 1.79E­05 1.89E­04 2.52E­03 ­1.49E­03
kg NMVOC
POCP 3.63E­03 1.33E­04 5.62E­05 4.91E­06 3.39E­05 5.22E­04 ­4.02E­04
eq
ADPE kg Sb eq 6.5E­07 3.63E­09 6.77E­09 8.06E­12 3.52E­10 4.62E­09 ­6.06E­08
ADPF MJ 3.3E+01 6.73E­01 3.61E­01 3.81E­03 1.66E­01 5.52E­01 ­6.7E+00
m3 world eq
WDP 4.6E­01 4.52E­04 2.1E­02 5.27E­07 2.3E­05 1.57E­01 ­3.7E­02
deprived
GWP = Global warming potential; ODP = Depletion potential of the stratospheric ozone layer; AP = Acidification potential of land and water; EP =
Eutrophication potential; POCP = Formation potential of tropospheric ozone photochemical oxidants; ADPE = Abiotic depletion potential for non­fossil
resources; ADPF = Abiotic depletion potential for fossil resources; WDP = Water (user) deprivation potential)
RESULTS OF THE LCA ­ INDICATORS TO DESCRIBE RESOURCE USE according to EN 15804+A2: 1 kg of dispersion­based
product, group 1
Parameter Unit A1­A3 A4 A5 C1 C2 C3 D
PERE MJ 4.66E+00 3.79E­02 6.43E­01 1.2E­05 5.25E­04 9.36E­02 ­1.32E+00
PERM MJ 5.85E­01 0 ­5.85E­01 0 0 0 0
PERT MJ 5.25E+00 3.79E­02 5.83E­02 1.2E­05 5.25E­04 9.36E­02 ­1.32E+00
PENRE MJ 1.78E+01 6.74E­01 1.31E+00 3.81E­03 1.67E­01 1.49E+01 ­6.7E+00
PENRM MJ 1.53E+01 0 ­9.53E­01 0 0 ­1.43E+01 0
PENRT MJ 3.3E+01 6.74E­01 3.62E­01 3.81E­03 1.67E­01 5.52E­01 ­6.7E+00
SM kg 0 0 0 0 0 0 0
RSF MJ 0 0 0 0 0 0 0
NRSF MJ 0 0 0 0 0 0 0
FW m3 1.19E­02 4.38E­05 5.03E­04 2.16E­08 9.41E­07 3.7E­03 ­1.53E­03
PERE = Use of renewable primary energy excluding renewable primary energy resources used as raw materials; PERM = Use of renewable primary
energy resources used as raw materials; PERT = Total use of renewable primary energy resources; PENRE = Use of non­renewable primary energy
excluding non­renewable primary energy resources used as raw materials; PENRM = Use of non­renewable primary energy resources used as raw
materials; PENRT = Total use of non­renewable primary energy resources; SM = Use of secondary material; RSF = Use of renewable secondary fuels;
NRSF = Use of non­renewable secondary fuels; FW = Use of net fresh water
RESULTS OF THE LCA – WASTE CATEGORIES AND OUTPUT FLOWS according to EN 15804+A2:
1 kg of dispersion­based product, group 1
Parameter Unit A1­A3 A4 A5 C1 C2 C3 D
HWD kg 8.74E­09 3.14E­08 1.23E­10 3.7E­13 1.62E­11 1.77E­09 ­2.66E­09
NHWD kg 1.3E­02 1.03E­04 2.35E­03 3.9E­07 1.7E­05 1.36E­01 ­2.94E­03
RWD kg 6.56E­04 8.34E­07 8.31E­06 4.09E­09 1.79E­07 2.51E­05 ­4.51E­04
CRU kg 0 0 0 0 0 0 0
MFR kg 0 0 0 0 0 0 0
MER kg 0 0 0 0 0 0 0
EEE MJ 0 0 2.77E­01 0 0 0 0
EET MJ 0 0 5.01E­01 0 0 0 0
6 Environmental Product Declaration ­ fischerwerke GmbH & Co. KG ­ FiAM Plus
HWD = Hazardous waste disposed; NHWD = Non­hazardous waste disposed; RWD = Radioactive waste disposed; CRU = Components for re­use;
MFR = Materials for recycling; MER = Materials for energy recovery; EEE = Exported electrical energy; EET = Exported thermal energy
RESULTS OF THE LCA – additional impact categories according to EN 15804+A2­optional:
1 kg of dispersion­based product, group 1
Parameter Unit A1­A3 A4 A5 C1 C2 C3 D
Disease
PM ND ND ND ND ND ND ND
incidence
IR kBq U235 eq ND ND ND ND ND ND ND
ETP­fw CTUe ND ND ND ND ND ND ND
HTP­c CTUh ND ND ND ND ND ND ND
HTP­nc CTUh ND ND ND ND ND ND ND
SQP SQP ND ND ND ND ND ND ND
PM = Potential incidence of disease due to PM emissions; IR = Potential Human exposure efficiency relative to U235; ETP­fw = Potential comparative
Toxic Unit for ecosystems; HTP­c = Potential comparative Toxic Unit for humans (cancerogenic); HTP­nc = Potential comparative Toxic Unit for humans
(not cancerogenic); SQP = Potential soil quality index
Potential Human exposure efficiency relative to U235, Disclaimer 1 – This impact category deals mainly with the eventual impact of low
dose ionizing radiation on human health of the nuclear fuel cycle. It does not consider effects due to possible nuclear accidents,
occupational exposure nor radioactive waste disposal in underground facilities. Potential ionizing radiation from the soil, radon and
(from) some construction materials are also not measured by this indicator.
ADP minerals & metals, ADP fossil, WDP, ETF­fw, HTP­c, HTP­nc, SQP, Disclaimer 2 – The results of this environmental impact
indicator shall be used with care as the uncertainties on these results are high or as there is limited experience with the indicator.
Additional environmental impact indicators (suggested by EN15804, table 4) are not declared in the EPD. The results of this
environmental impact indicator shall be used with care as the uncertainties on these results are high and as there is limited experience
with the indicator (see ILCD classification in EN 15804, table 5). For this reason, results based on these indicators are not considered
suitable for a decision­making process and are thus not declared in the EPD.
6. LCA: Interpretation
The majority of impacts are associated with the production Demand – Renewable (PERT) generally represents a small
phase (A1­A3). The most significant contribution to the percentage of the production phase primary energy demand
production phase impacts is the upstream production of raw with the bulk of the demand coming from non­renewable
materials as the main driver. Another contributor in the energy resources.
production phase, in the category of Photochemical ozone
formation (POCP),
is the plastic used as a packaging material. Emissions Transportation to the construction site (A4) and the installation
associated with the process (A5) make a low contribution to all impacts. Climate
manufacturing of products also have some influence on Ozone change from land­use change is the only indicator influenced
Depletion Potential by transport processes, due to the diesel production used as
(ODP) in the production phase. In all EPDs, CO is the most fuel because part of this diesel has been produced from bio­
2
important contributor to Global Warming Potential (GWP). For based raw materials.
the Acidification Potential (AP), NOx and SO contribute the
2
largest share.
The installation phase influence mainly climate change
indicators, due to the impact related to the incineration
processes used for packaging waste treatment and residual
The majority of life cycle energy consumption takes place
product treatment (1 % of the total mass).
during the production phase (A1­A3). Significant contributions
to Primary Energy Demand – Non­renewable (PENRT) come
from the energy resources used in the production of raw
The end­of­life phases influence climate change indicators, due
materials. The largest contributor to Primary Energy Demand –
to the thermal treatment process of the dispersion­based
Renewable (PERT) impacts comes from the consumption of
product occurring in the C3 module.
renewable energy resources required for the generation and
supply of electricity. It should be noted that Primary Energy
7. Requisite evidence
VOC Emissions
fischer FiAM Plus was tested according to Indoor Air Comfort
GOLD by Eurofins Product Testing A/S in Denmark (test report
from 10.02.2023).
Selected values for AgBB are shown in table 7.1, compliance
Table 7.1: AgBB overview of results (28 days [µg/m³])
with different regulations is shown in table 7.2.
7 Environmental Product Declaration ­ fischerwerke GmbH & Co. KG ­ FiAM Plus
Name Value Unit Name Value Unit
TVOC (C6 ­ C16) 5 μg/m3 Indoor Air Comfort GOLD Pass ­
Sum SVOC (C16 ­ C22) 5 μg/m3 French VOC regulation A+ ­
R (dimensionless) ­ ­ ABG/AgBB Pass ­
VOC without NIK 5 μg/m3 Belgian Regulation Pass ­
Carcinogenic Substances 1 μg/m3 Blue Angel (DE­UZ 123) Pass ­
EMICODE EC 1 PLUS ­
Table 7.2: Results of different VOC evaluations BREEAM International Exemplary Level ­
BREEAM NOR Exemplary Level ­
8. References
EN 1062­3 EN15804:2019+A2+AC, Sustainability of construction works —
EN 1062­3:2008­04, Paints and varnishes ­ Coating materials Environmental Product
and coating systems for exterior masonry and concrete ­ Part 3: Declarations — Core rules for the product category of
Determination of liquid water construction products.
permeability
EN 16516
EN 1062­6 EN 16516:2017 Construction products ­ Assessment of release
EN 1062­6:2002­10, Paints and varnishes ­ Coating materials of dangerous substances ­
and coating systems for exterior masonry and concrete ­ Part 6: Determination of emissions into indoor air
Determination of carbon dioxide permeability
EN ISO 17025
DIN EN ISO 1183­1 EN ISO 17025:2018­03 General requirements for the
DIN EN ISO 1183­1:2019­09, Plastics ­ Methods for competence of testing and calibration laboratories
determining the density of non­cellular plastics ­ Part 1:
Immersion method, liquid pycnometer method and titration EN ISO 17178
method EN ISO17178:2020, Adhesives ­ Adhesives for bonding parquet
to subfloor ­ Test
EN 1504­2 methods and minimum requirements
EN 1504­2:2004­10, Products and systems for the protection
and repair of concrete structures ­ Definitions, requirements, EN ISO 22636
quality control and evaluation of EN ISO22636:2020, Adhesives ­ Adhesives for floor coverings ­
conformity ­ Part 2: Surface protection systems for concrete Requirements for
mechanical and electrical performance
EN 1542
EN1542:1999­07, Products and systems for the protection and ASTM E84
repair of concrete ASTM E84­21a, Standard Test Method for Surface
structures ­ Test methods ­ Measurement of bond strength by BurningCharacteristics of Building Materials
pull­off
EAD 030352­00­0503
EN ISO 7783­1/­2 EAD030352­00­0503:2019­01, Watertight covering kits for wet
EN ISO 7783­1/­2:20­02, Paints and varnishes ­ Determination room floors and or walls Part 1: Liquid Applied Coverings with
of water­vapour transmission properties ­ Cup method or without wearing surface Part 2: Kits based on flexible sheets
Part 3: Kits based on inherently watertight boards
EN 12004
EN12004:2012, EAD 350454­00­1104
Adhesives for ceramic tiles EAD 350454­00­1104:2017­09, Fire stopping and fire sealing
products ­ penetration seals
EN 12004­2
EN12004­2:2017, Adhesives for ceramic tiles ­ Part 2: Test EAD 350141­00­1106
methods EAD 350141­00­1106:2017­09, Fire stopping and fire sealing
products ­ linear joint and gap seals
DIN EN 13501­­1
DIN EN 13501­­1:2019­­05, Fire classification of ETA­23/0163
constructionproducts and building elements ­ Part 1: ETA­­23/­0163, European Technical Approval for fischer FiAM
Classification usingdata from reaction to fire tests Plus for penetration seals
ISO 14001 ETA­23/0165
DIN EN ISO 14001:2015­­11, Environmental ETA­­23­/0166, European Technical Approval for fischer FiAM
managementsystems ­ Requirements with guidance for use Plus for linear gap seals
ISO 14025 UL723­11
DIN EN ISO14025:2011­10, Environmental labels and UL723­­11, Test for Surface Burning Characteristics of
declarations — Type III environmental BuildingMaterials
declarations — Principles and procedures
(EU) No 528/2012
EN 15804 Biocidal Products Regulation (EU) No 528/2012 of the
8 Environmental Product Declaration ­ fischerwerke GmbH & Co. KG ­ FiAM Plus
European Parliament and of the of GaBi 10 data sets http://documentation.gabi­software.com/,
Council of 22 May 2012 concerning the making available on the 2020
market and use of
biocidal products (current consolidated version: 2021­06) German AgBB
Committee for Health­related Evaluation of Building Products:
2000/532/EC health­related evaluation of
Commission decision dated 3 May 2000 replacing decision emissions of volatile organic compounds (VOC and SVOC)
94/3/EC on a waste directory in from building products;
accordance with Article 1 a) of Council Directive 75/442/EEC on status: June 2012
waste and www.umweltbundesamt.de/produkte/bauprodukte/agbb.htm
Council decision 94/904/EC on a directory of hazardous waste
in terms of IBU 2021
Article 1, paragraph 4 of Directive 91/689/EEC on hazardous Institut Bauen und Umwelt e.V.: General Instructions for the
waste EPD programme of Institut Bauen und Umwelt e.V. EPD
programme. Version 2.0. Berlin: Institut Bauen und Umwelt
Belgian Royal Decree C­2014/24239 e.V., 2021
Belgisch Staatsblad 8 MEI 2014, p. 60603. — Koninklijk besluit www.ibu­epd.com
tot vaststelling
van de drempelniveaus voor de emissies naar het binnenmilieu Indoor Air Comfort
van bouwproducten Product certification by Eurofins, Hamburg, Germany
voor bepaalde geoogde gebruiken www.eurofins.com .
Blue Angel PCR Part A
Environmental label organised by the federal government of Product Category Rules for Building­Related Products and
Germany www.blauer­engel.de Services, Part A: Calculation
Rules for the Life Cycle Assessment and Requirements on the
Candidate list Project report,
Candidate List of substances of very high concern for Version 1.1, Institut Bauen und Umwelt e.V., 2021­01
Authorisation, published in accordance
with Article 59(10) of the REACH Regulation, ECHA, PCR Part B
www.echa.europa.eu/candidate­list­table Product Category Rules for Construction Products. Part B:
Dispersion adhesives and primers for floor coverings, Version
CPR 1.7, 2019.
CPR Regulation (EU) No 305/2011 of the European Parliament
and of the Council of 9 March 2011 laying down harmonised REACH
conditions for the marketing of construction products Directive (EG) No. 1907/2006 of the European Parliament and
and repealing Council Directive 89/106/EEC of the Council dated 18 December 2006 on the registration,
evaluation, approval and restriction of chemical
Decopaint Directive substances (REACH), for establishing a European Agency for
Directive 2004/42/CE of the European Parliament and the chemical substances,
council of 21 April 2004 on the for amending Directive 1999/45/EC and for annulment of
limitation of emissions of volatile organic compounds due to the Directive (EEC) No.
use of organic 793/93 of the Council, Directive (EC) No. 1488/94 of the
solvents in certain paints and varnishes and vehicle refinishing Commission, Guideline
products and 76/769/EEC of the Council and Guidelines 91/155/EEC,
amending Directive 1999/13/EC 93/67/EEC, 93/105/EC and
2000/21/EC of the Commission.
EMICODE
EMICODE, GEV – Gemeinschaft Emissionskontrollierte UL
Verlegewerkstoffe, Klebstoffe und Bauprodukte e. V. UL Solutions, Northbrook Illinois USA, www.ul.com
(pub.).www.emicode.de The literature referred to in the Environmental Product
Declaration must be listed in full.Standards already fully quoted
GaBi 10 software & documentation in the EPD do not need to be listed here again.
Data base for Life Cycle Engineering LBP, University of The current version of PCR Part A and PCR Part B of the PCR
Stuttgart and Sphera, documentation document on which they are based must be referenced.
9 Environmental Product Declaration ­ fischerwerke GmbH & Co. KG ­ FiAM Plus
Publisher
Institut Bauen und Umwelt e.V. +49 (0)30 3087748­ 0
Hegelplatz 1 info@ibu­epd.com
10117 Berlin www.ibu­epd.com
Germany
Programme holder
Institut Bauen und Umwelt e.V. +49 (0)30 3087748­ 0
Hegelplatz 1 info@ibu­epd.com
10117 Berlin www.ibu­epd.com
Germany
Author of the Life Cycle Assessment
Sphera Solutions GmbH +49 711 341817­0
Hauptstraße 111­ 113 info@sphera.com
70771 Leinfelden­Echterdingen www.sphera.com
Germany
Owner of the Declaration
fischerwerke GmbH & Co. KG +49 (0)7443 12­0
Klaus­Fischer­Straße 1 info@fischer.de
72178 Waldachtal www.fischer.de
Germany
Industrieverband Klebstoffe e.V +49 (0)211 67931­10
Völklinger Straße 4 info@klebstoffe.com
40219 Düsseldorf www.klebstoffe.com
Germany
Deutsche Bauchemie e.V. +49 (0)69 2556­1318
Mainzer Landstr. 55 info@deutsche­bauchemie.de
60329 Frankfurt www.deutsche­bauchemie.de
Germany
FEICA ­ Association of the European Adhesive and +32 (0)267 673 20
Sealant Industry info@feica.eu
Rue Belliard 40 box 10 www.feica.eu
1040 Brussels
Belgium
EFCC ­ European Federation for Construction +32289720­39
Chemicals info@efcc.be
Boulevard du Triomphe 172 www.efcc.eu
1160 Brussels
Belgium
10 Environmental Product Declaration ­ fischerwerke GmbH & Co. KG ­ FiAM Plus
