ENVIRONMENTAL PRODUCT DECLARATION
as per ISO 14025 and EN 15804+A2
Owner of the Declaration
Programme holder Institut Bauen und Umwelt e.V. (IBU)
Publisher Institut Bauen und Umwelt e.V. (IBU)
Declaration number EPD-USG-20220126-IAA1-EN
Issue date 07.07.2022
Valid to 06.07.2027
AQUAPANEL® Cement Board Outdoor - Site Volos (GR)
Knauf AQUAPANEL GmbH & Co. KG
www.ibu-epd.com | https://epd-online.com
Umwelt Produktdeklaration Name des Herstellers – Name des Produkts
1. General Information
Knauf AQUAPANEL GmbH & Co. KG AQUAPANEL® Cement Board
Outdoor
Programme holder Owner of the declaration
IBU – Institut Bauen und Umwelt e.V. Knauf AQUAPANEL GmbH & Co. KG
Hegelplatz 1 Zur Helle 11
10117 Berlin 58638 Iserlohn
Germany Deutschland
Declaration number Declared product / declared unit
EPD-USG-20220126-IAA1-EN 1 m² AQUAPANEL® Cement Board Outdoor with a
thickness of 12.5 mm.
This declaration is based on the product Scope:
category rules: This Environmental Product Declaration refers to
Fibre cement / Fibre concrete, 01.2019 AQUAPANEL® Cement Board Outdoor from the
(PCR checked and approved by the SVR) production facility in Volos, Greece.
Issue date The owner of the declaration shall be liable for the
07.07.2022 underlying information and evidence; the IBU shall not
be liable with respect to manufacturer information, life
cycle assessment data and evidences.
Valid to
The EPD was created according to the specifications
06.07.2027
of EN 15804+A2. In the following, the standard will be
simplified as EN 15804.
Verification
The standard EN 15804 serves as the core PCR
Independent verification of the declaration and data
according to ISO 14025:2011
Dipl. Ing. Hans Peters internally x externally
(chairman of Institut Bauen und Umwelt e.V.)
Dr. Alexander Röder Prof. Dr. Birgit Grahl
(Managing Director Institut Bauen und Umwelt e.V.)) (Independent verifier)
2. Product
2.1 Product description/Product definition
Cement-bound, mineral building panel with Constructional data
twodimensional lattice structures consisting of Name Value Unit
longitudinal and transverse glass fibres for outdoor Thermal conductivity acc to ISO
0.35 W/(mK)
use. 10456
The AQUAPANEL® Cement Board Outdoor is a CPR Water vapour diffusion resistance
66 -
product with European Technical Assessment (ETA). factor acc. to ISO 12572
The placing on the market of the product in the Swelling (air-dry to water-
0.23 mm/m
European Union/European Free Trade Association saturated) acc. to EN 318
(EU / EFTA) (with the exception of Switzerland) is also Gross density acc. to /EN 12467/ 1150 kg/m3
subject to Regulation (EU) No 305/2011 (CPR). The Tensile strength acc. to EN 319 0.65 N/mm2
product requires a declaration of performance in Flexural strength acc. to EN
consideration of ETA-07/0173, dated 11.10.2017 and 12467 >=7 N/mm2
the CE marking. Coefficient of thermal expansion 7 10-6K-1
For the use of the product, the respective national
regulations apply.
Product according to the CPR, based on an ETA:
 Performance data of the product in
2.2 Application
accordance with the declaration of
The "AQUAPANEL® Cement Board Outdoor" building
performance with respect to its essential
board is used as a non-load-bearing wall element in
exteriors characteristics according to ETA-07/0173,
11.10.2017.
2.3 Technical Data  Voluntary data: source, Technical Data Sheet,
08/17 (www.aquapanel.com).
2 Environmental Product Declaration Knauf AQUAPANEL GmbH & Co. KG – AQUAPANEL® Cement Board Outdoor - Site
Volos
(not part of CE-marking) do not meet the requirements as well as any edge
trimmings produced during the final processing of the
2.4 Delivery status slabs are returned to the manufacturing process as
The panels are sold in widths of 900 mm and in raw material.
lengths of 1200/1250/2400/2500 mm. The layer b) Optimization of energy consumption: A high degree
thickness is 12.5 mm. of automation in production enables optimal process
parameters to be maintained, thus minimizing
2.5 Base materials/Ancillary materials unnecessary energy consumption. This applies in
particular to the expansion of the perlite raw material
Name Value Unit
Cement 20-30 Mass-% 2.8 Product processing/Installation
Limestone 30-50 Mass-% Knauf Aquapanel GmbH & Co. KG provides technical
Perlite 5-20 Mass-% data sheets for the cement-bonded building boards.
Recyclate 0-10 Mass-% This information is available in printed form as well as
Glas fibre scrim <2 Mass-% at www.aquapanel.com.
Hydrophobic agent <1 Mass-%
The boards can be mechanically fastened or glued.
The product contains substances on the ECHA The processing can be carried out with commercially
Candidate List of Substances of Very High Concern available tools.
(SVHC) (date 04.05.2021) above 0.1% by mass: no.
The product contains other carcinogenic, mutagenic, 2.9 Packaging
reprotoxic (CMR) substances of category 1A or 1B, The cement-bonded building board with glass grid
which are not on the candidate list, above 0.1% by reinforcement is delivered on a returnable Euro pallet
mass in at least one sub-product: no. secured with metal strapping
Biocidal products have been added to the present
construction product or it has been treated with
biocidal products (it is therefore a treated product in 2.10 Condition of use
the sense of the Biocidal Products Regulation (EU) No No changes in material composition occur during
528/2012): no. service life.
2.6 Manufacture 2.11 Environment and health during use
The aggregates and binders are stored in silos outside During the service life, there are no environmental and
the production hall. The raw materials for the panel health effects. The results of the Volatile Organic
core are dosed over belt scales and loss-in-weight Compound (VOC) analysis all remained below the
feeders according to formula and transported to the respective detection limit (see chapter 7.3). There is no
weighing container via a central conveyor. The binder release of chromium (VI)-containing substances. There
for the production of the cover layer is transported are no hazards to water, air or soil. In use, the
directly via a screw conveyor to the slurry production ingredients of the products are firmly bound. Dust
unit. The glass fabrics required for production are emissions are not possible.
stored in the basement of the production hall. The
expansion of the perlite rock takes place at the Volos 2.12 Reference service life
site. The dry mixture in the weighing container is From experience, a service life of approximately 50
emptied into the compulsory mixer underneath and years can be achieved when used as intended.
water is added according to the formula. The core
mixture is mixed homogeneously and earth-moist and Description of the influences on the ageing of the
then conveyed by belt to the forming station. At the product when applied in accordance with the rules of
same time, the slurry for the surface layer is premixed technology.
homogeneously and conveyed by screw pumps
through hoses to the forming station. In the forming
station, the 3-layer element is produced by continuous 2.13 Extraordinary effects
extrusion and cut in the subsequent cutting apparatus
to the appropriate length. The tailored boards are Fire
hardened in the shelf storage. Non-combustible building material of building material
The production process is DIN EN ISO 9001 certified. class A1 acc to EN 13501-1.
2.7 Environment and health during Fire protection
manufacturing Name Value
According to Regulation (EC) No 1907/2006, cement Building material class A1
and cement-containing mixtures may not be used or
placed on the market if the content of soluble Water
chromium(VI) in the dry mass of the cement after Chromium elution is to be expected in case of
hydration is more than 2 mg/kg (0.0002 %). Only unforeseen effects of water in non-relevant quantities
lowchromate cements are used in the production (see chapter 7.2). Further elutions of other heavy
process. metals are not expected.
Apart from the legal requirements, no further special
measures are necessary. Mechanical destruction
No sharp break edges are created upon mechanical
Further environmental protection measures in the destruction.
production process:
a) Minimization of waste: Both manufactured slabs that
3 Environmental Product Declaration Knauf AQUAPANEL GmbH & Co. KG – AQUAPANEL® Cement Board Outdoor - Site
Volos
2.14 Re-use phase and demolition waste other than those falling under
Once used, the products are practically un-reusable, 170901, 170902 and 170903 is recommended.
but are suitable for recycling as filling material if fully
separated. 2.16 Further information
For further information visit: www.aquapanel.com.
2.15 Disposal
According to AVV AQUAPANEL® Cement Board
Rooftop, the waste code 170904 mixed construction
3. LCA: Calculation rules
3.1 Declared Unit consideration. Due to the frequent reuse, the
The declared unit of the study is 1 m² AQUAPANEL® proportion to be taken into account for a declared unit
Cement Board Outdoor with a thickness of 12.5 mm. is very low and does not have a significant share in the
result. Furthermore, the section of metal strapping
Declared unit occurs during pallet loading. In relation to a declared
Name Value Unit unit, the share is <0.1% of the total mass input.
Declared Unit 1 m² An application of the cut-off criteria beyond the
Gross density * 1150 kg/m3 abovementioned processes was not necessary.
Grammage 16 kg/m2
Layer thickness 0.0125 m 3.5 Background data
* The density according to EN 12467 is the density The background data used was completely obtained
after complete drying. Therefore, the data in the above from the GaBi-ts software or can be traced back to it.
table on surface weight at delivery and the bulk GaBi (Content Version 2021.2, Service Pack 40) was
density do not correlate, used to calculate the LCA.
3.6 Data quality
3.2 System boundary All background data records relevant for the calculation
Within the scope of the conducted LCA, the production were provided by the declaration holder and processed
or provision and transport of the preliminary with the database of the accounting software GaBi ts.
products/raw materials as well as the production of the The manufacturer-specific data used is from 2020. All
final product (A1-A3) are taken into account. material and energy flows were recorded in full and
Furthermore, the end-of-life phase (C1-C4) is were taken into account in the processes described in
considered using technical scenarios. chapter 3.2.
The data of the cement board production was
determined at the production site. The recipe and the 3.7 Period under review
raw materials used, the electrical energy used and all The review period for the data collection is 2020.
direct production waste were taken into account in the
balancing. Within phase A2, all specific transport 3.8 Allocation
routes of the educts were stored. Allocation in the factory. The data specification was
made regarding the actual output in the reference
3.3 Estimates and assumptions period based on the produced area. Regarding the
With the exception of the technical scenarios (Chapter offcut material there is a closed loop.
4), no estimates or assumptions were made in the
study. 3.9 Comparability
Basically, a comparison or an evaluation of EPD data
3.4 Cut-off criteria is only possible if all the data sets to be compared
In the LCA, the cut-off criteria for a release agent was were created according to EN 15804 and the building
applied in the area of production. The material context, respectively the product-specific
corresponds to <0.08 % of the mass input for the characteristics of performance, are taken into account.
declared unit. The use of the wooden pallets used for
storage and transport is also cut off within the The background data was taken from the GaBi ts
software (Content Version 2021.2, Service Pack 40).
4. LCA: Scenarios and additional technical information
Characteristic product properties excavator (incl. diesel), depending on the mass to be
Information on biogenic Carbon moved (declared unit).
AQUAPANEL® Cement Board Outdoor is almost Module C2 – Transport for waste management
exclusively composed of inorganic materials. The The transport of the deconstructed material is
proportion of biogenic carbon in the total mass of the assumed to take place with one truck as a German
product is less than 1 %. fleet average to an inert material landfill as mixed
construction waste. The transport distance is assumed
to be 100 km.
Module C1 - Deconstruction and demolition Module C3 - Waste management for
The deconstruction is carried out mechanically and reuse, recovery and/or recycling
unspecifically with an excavator (100 kW), related to The product under consideration can be used as bulk
the product under consideration. The scenario and fill material if separated by type. In practice, the
considers the impacts caused by the operation of the deconstructed structure is not separated by type, so
4 Environmental Product Declaration Knauf AQUAPANEL GmbH & Co. KG – AQUAPANEL® Cement Board Outdoor - Site
Volos
that a pure inert material landfill is assumed in this
scenario.
Module C4 - Disposal
The product under consideration is disposed of as part
of mixed construction waste in an inert landfill. No
consideration is given to energy credits from possible
landfill gas use, as the product consists almost
exclusively of inorganic materials.
Module D - Reuse, recovery and/or recycling
potentials
Due to the assumed landfilling of inert materials, a
consideration of credits is not possible.
5 Environmental Product Declaration Knauf AQUAPANEL GmbH & Co. KG – AQUAPANEL® Cement Board Outdoor - Site
Volos
5. LCA: Results
The results of the life cycle assessment of the AQUAPANEL® Cement Board Outdoor for the life cycle phases
considered (A1-A3, C1-C4, D) are presented below. The characterisation factors of EK-JRC specified by EN
15804 were used.
DESCRIPTION OF THE SYSTEM BOUNDARY (X = INCLUDED IN LCA; ND = MODULE OR INDICATOR NOT
DECLARED; MNR = MODULE NOT RELEVANT)
BENEFITS AND
CONSTRUCTI LOADS
PRODUCT STAGE ON PROCESS USE STAGE END OF LIFE STAGE BEYOND THE
STAGE SYSTEM
BOUNDARIES
6 Environmental Product Declaration Knauf AQUAPANEL GmbH & Co. KG – AQUAPANEL® Cement Board Outdoor - Site
Volos
lairetam
waR
ylppus tropsnarT
gnirutcafunaM
eht
morf
tropsnarT
etis
eht
ot
etag
ylbmessA esU
ecnanetniaM
riapeR
tnemecalpeR tnemhsibrufeR
ygrene
lanoitarepO esu
retaw
lanoitarepO esu
noitcurtsnoc-eD
noitilomed tropsnarT
gnissecorp
etsaW
lasopsiD -esueR -yrevoceR -gnilcyceR laitnetop
A1 A2 A3 A4 A5 B1 B2 B3 B4 B5 B6 B7 C1 C2 C3 C4 D
X X X ND ND ND ND MNR MNR MNR ND ND X X X X X
RESULTS OF THE LCA - ENVIRONMENTAL IMPACT according to EN 15804+A2: 1 m² AQUAPANEL®
Cement Board Outdoor
Core Indicator Unit A1 A2 A3 C1 C2 C3 C4 D
GWP-total [kg CO2-Eq.] 3.73 0.09 0.62 0.01 0.10 0.00 0.23 0.00
GWP-fossil [kg CO2-Eq.] 3.70 0.09 0.62 0.01 0.10 0.00 0.25 0.00
GWP-biogenic [kg CO2-Eq.] 3.00E-2 -9.09E-5 1.40E-3 -4.42E-4 4.00E-5 0.00E+0 -1.97E-2 0.00E+0
GWP-luluc [kg CO2-Eq.] 1.63E-3 6.78E-4 1.09E-4 4.18E-5 4.16E-4 0.00E+0 7.17E-4 0.00E+0
ODP [kg CFC11-Eq.] 1.52E-14 2.02E-17 4.62E-15 2.45E-18 2.44E-17 0.00E+0 9.91E-16 0.00E+0
AP [mol H+-Eq.] 8.79E-3 5.41E-4 1.13E-3 4.92E-5 5.73E-4 0.00E+0 1.78E-3 0.00E+0
EP-freshwater [kg P4-Eq.] 2.90E-6 2.48E-7 1.83E-7 2.17E-8 2.16E-7 0.00E+0 4.26E-7 0.00E+0
EP-marine [kg N-Eq.] 2.43E-3 2.65E-4 2.19E-4 2.32E-5 2.81E-4 0.00E+0 4.58E-4 0.00E+0
EP-terrestrial [mol N-Eq.] 2.66E-2 2.92E-3 2.39E-3 2.57E-4 3.12E-3 0.00E+0 5.03E-3 0.00E+0
POCP [kg NMVOC-Eq.] 7.19E-3 5.32E-4 6.67E-4 6.49E-5 5.37E-4 0.00E+0 1.39E-3 0.00E+0
ADPE [kg Sb-Eq.] 3.04E-7 7.54E-9 7.27E-8 8.29E-10 8.25E-9 0.00E+0 2.23E-8 0.00E+0
ADPF [MJ] 29.30 1.16 8.50 0.13 1.32 0.00 3.25 0.00
[m³ world-Eq
WDP 2.60E-1 8.12E-4 1.12E-1 4.30E-5 4.28E-4 0.00E+0 2.60E-2 0.00E+0
deprived]
GWP = Global warming potential; ODP = Depletion potential of the stratospheric ozone layer; AP = Acidification potential of land and water; EP =
Caption Eutrophication potential; POCP = Formation potential of tropospheric ozone photochemical oxidants; ADPE = Abiotic depletion potential for non-
fossil resources; ADPF = Abiotic depletion potential for fossil resources; WDP = Water (user) deprivation potential
RESULTS OF THE LCA - INDICATORS TO DESCRIBE RESOURCE USE according to EN 15804+A2: 1 m²
AQUAPANEL® Cement Board Outdoor
Indicator Unit A1 A2 A3 C1 C2 C3 C4 D
PERE [MJ] 4.34 0.06 1.12 0.01 0.08 0.00 0.43 0.00
PERM [MJ] 0.00 0.00 0.00 0.00 0.00 0.00 0.00 0.00
PERT [MJ] 4.34 0.06 1.12 0.01 0.08 0.00 0.43 0.00
PENRE [MJ] 29.50 1.16 8.50 0.13 1.32 0.00 3.26 0.00
PENRM [MJ] 0.00 0.00 0.00 0.00 0.00 0.00 0.00 0.00
PENRT [MJ] 29.50 1.16 8.50 0.13 1.32 0.00 3.26 0.00
SM [kg] 0.05 0.00 0.00 0.00 0.00 0.00 0.00 0.00
RSF [MJ] 2.07 0.00 0.00 0.00 0.00 0.00 0.00 0.00
NRSF [MJ] 3.93 0.00 0.00 0.00 0.00 0.00 0.00 0.00
FW [m³] 7.22E-2 7.52E-5 1.78E-3 6.91E-5 6.88E-5 0.00E+0 8.20E-4 0.00E+0
PERE = Use of renewable primary energy excluding renewable primary energy resources used as raw materials; PERM = Use of
renewable primary energy resources used as raw materials; PERT = Total use of renewable primary energy resources; PENRE = Use of
non-renewable primary energy excluding non-renewable primary energy resources used as raw materials; PENRM = Use of non-
Caption
renewable primary energy resources used as raw materials; PENRT = Total use of non-renewable primary energy resources; SM = Use
of secondary material; RSF = Use of renewable secondary fuels; NRSF = Use of non-renewable secondary fuels; FW = Use of net fresh
water
RESULTS OF THE LCA – WASTE CATEGORIES AND OUTPUT FLOWS according to EN 15804+A2:
1 m² AQUAPANEL® Cement Board Outdoor
Indicator Unit A1 A2 A3 C1 C2 C3 C4 D
HWD [kg] 3.38E-8 6.21E-11 1.66E-9 4.95E-9 4.93E-8 0.00E+0 4.96E-8 0.00E+0
NHWD [kg] 6.56E-2 1.82E-4 2.58E-3 2.33E-5 2.32E-4 0.00E+0 1.64E+1 0.00E+0
RWD [kg] 8.79E-4 2.16E-6 2.76E-5 1.40E-7 1.39E-6 0.00E+0 3.70E-5 0.00E+0
CRU [kg] 0.00 0.00 0.00 0.00 0.00 0.00 0.00 0.00
MFR [kg] 0.00 0.00 0.00 0.00 0.00 0.00 0.00 0.00
MER [kg] 0.00 0.00 0.00 0.00 0.00 0.00 0.00 0.00
EEE [MJ] 0.00 0.00 0.00 0.00 0.00 0.00 0.00 0.00
EET [MJ] 0.00 0.00 0.00 0.00 0.00 0.00 0.00 0.00
HWD = Hazardous waste disposed; NHWD = Non-hazardous waste disposed; RWD = Radioactive waste disposed; CRU = Components
Caption for re-use; MFR = Materials for recycling; MER = Materials for energy recovery; EEE = Exported electrical energy; EEE = Exported
thermal energy
RESULTS OF THE LCA – additional impact categories according to EN 15804+A2-optional:
1 m² AQUAPANEL® Cement Board Outdoor
Indicator Unit A1 A2 A3 C1 C2 C3 C4 D
[Disease
PM ND ND ND ND ND ND ND ND
Incidence]
[kBq U235-
IRP ND ND ND ND ND ND ND ND
Eq.]
ETP-fw [CTUe] ND ND ND ND ND ND ND ND
HTP-c [CTUh] ND ND ND ND ND ND ND ND
HTP-nc [CTUh] ND ND ND ND ND ND ND ND
SQP [-] ND ND ND ND ND ND ND ND
PM = Potential incidence of disease due to PM emissions; IR = Potential Human exposure efficiency relative to U235; ETP-fw = Potential
Caption comparative Toxic Unit for ecosystems; HTP-c = Potential comparative Toxic Unit for humans (cancerogenic); HTP-nc = Potential
comparative Toxic Unit for humans (not cancerogenic); SQP = Potential soil quality index
Disclaimer 1 – for the indicator “Potential Human exposure efficiency relative to U235”. This impact category
deals mainly with the eventual impact of low-dose ionizing radiation on human health of the nuclear fuel cycle. It
does not consider effects due to possible nuclear accidents, occupational exposure or radioactive waste disposal
in underground facilities. Potential ionizing radiation from the soil, radon and from some construction materials is
also not measured by this indicator.
Disclaimer 2 – for the indicators “abiotic depletion potential for non-fossil resources”, “abiotic depletion potential
for fossil resources”, “water (user) deprivation potential, deprivation-weighted water consumption”, “potential
comparative toxic unit for ecosystems”, “potential comparative toxic unit for humans – cancerogenic”, “Potential
comparative toxic unit for humans - not cancerogenic”, “potential soil quality index”. The results of this
environmental impact indicator shall be used with care as the uncertainties on these results are high as there is
limited experience with the indicator.
6. LCA: Interpretation
Based on the dominance analysis of the use of plant have only minor impacts. The effects of the
resources, it can be seen that the most climate production process in the plant itself are rather
effective impact in the case of AQUAPANEL® cement subordinate in terms of life cycle assessment and are
panels is the raw material procurement/raw material largely due to the electrical energy demand. The
processing (module A1). The mineral raw materials processes used here are largely mixing and moulding
used for this are extracted as a non-regenerative processes that have hardly any environmental impact.
resource and in some cases also thermally treated The drying process in the curing warehouse takes
(glass melting, cement burning). The CEM I cement place without the use of additional thermal energy due
used in the product contributes approx. 60 % of the to exothermic processes.
Global Warming Potential (GWP) and is due to the
energy-intensive burning process. The second major
influence on the global warming potential represents
the use of glass fabric. The impact in relation to the
overall result was calculated at 20 %. The production
process is responsible for 14 % and consists of both
the electrical energy demand (6.3 %) and the thermal
energy demand for the perlite expansion process (7.6
%).
In the other impact categories considered, raw material
procurement and raw material processing (A1),
especially that of mineral raw materials, also stand out
as relevant processes in the overall system, whereas
the transport of raw materials and production at the
7. Requisite evidence
out by the Institut für Baubiologie Rosenheim (IBR) in
7.1 Radioactivity August 2020. The determination in the original
The Activity Concentration Index (ACI) was determined substance was carried out according to ISO 17294-2,
to be 0.18. The tested product meets the official in the eluate according to DIN 38414-4.
guideline value of ACl <1 as well as the test condition Institut für Baubiologie Rosenheim GmbH Test
ACl <0.75 of the Institut für Baubiologie Rosenheim Report No. 3020-1166.
(IBR). Institute for Building Biology Rosenheim GmbH
Test Report No. 3020-1166 of December 2020. Heavy metal concentrations in the original
substance
7.2 Leaching Name Value Unit
A determination of the heavy metal concentration both Arsenic 1,6 mg/kg
in the original substance and in the eluate was carried Cadmium <0,3 mg/kg
7 Environmental Product Declaration Knauf AQUAPANEL GmbH & Co. KG – AQUAPANEL® Cement Board Outdoor - Site
Volos
Chromium 22,1 mg/kg
Copper 35,1 mg/kg AgBB overview of results (28 days [µg/m³])
Mercury <0,05 mg/kg Name Value Unit
Nickel 9,61 mg/kg TVOC (C6 - C16) 862 μg/m3
Lead 6,0 mg/kg Sum SVOC (C16 - C22) <5 μg/m3
Zinc <30 mg/kg R (dimensionless) 0.21 -
VOC without NIK <5 μg/m3
Heavy metal concentration in the eluate Carcinogenic Substances <1 μg/m3
Name Value Unit
Arsenic <0,01 mg/l AgBB overview of results (3 days [µg/m³])
Cadmium <0,0005 mg/l Name Value Unit
Chromium 0,0231 mg/l TVOC (C6 - C16) 808 μg/m3
Copper <0,005 mg/l Sum SVOC (C16 - C22) <5 μg/m3
Mercury <0,0001 mg/l R (dimensionless) 0.27 -
Nickel <0,005 mg/l VOC without NIK 23 μg/m3
Lead <0,005 mg/l Carcinogenic Substances <1 μg/m3
Zinc 0,072 mg/l Based on the measurement results and the
comparison of the specifications of the AgBB scheme
7.3 VOC emissions and the DIBt approval principles, no contamination of
The analysis of emissions of volatile organic the tested product by emissions of volatile organic
compounds (VOC) starting from the AQUAPANEL® compounds and in particular by formaldehyde is to be
Cement Board Rooftop was carried out in December expected; therefore, the use of the cement boards in
2020 by the Institut für Baubiologie Rosenheim (IBR) interior rooms of buildings is harmless in terms of VOC
and the results were documented in test report No. emissions.
3020-1166.
8. References
AgBB Fibre-cement flat sheets - Product specification and
Committee for Health-related evaluation of building test methods; German version EN
products/Auschuss zur gesundheitlichen Bewertung 2467:2012+A2:2018
von Bauprodukten
EN 13501-1
AVV DIN EN 13501-1:2010-01 Fire classification of
Ordinance on the European list of waste construction products and building elements - Part 1:
(Abfallverzeichnis-Verordnung - AVV), 10.12.2001. Classification using data from reaction to fire tests
Biocidal Products Regulation EN 15804
Regulation (EU) No 528/2012 of the European EN 15804:2012+A2:2019, Sustainability of
Parliament and of the Council of 22 May 2012 construction works - Environmental product
concerning the making available on the market and declarations - Core rules for the product category of
use of biocidal products Text with EEA relevance. construction products
DIN 38414-4 ETA-07/0173
DIN 38414-4:1984-10, German standard methods for declaration of performance in consideration of ETA-
the examination of water, wastewater and sludge; 07/0173 and the CE marking, dated 11.10.2017.
sludge and sediments (group S); determination of
leachability by water (p 4). GaBi ts
GaBi ts: Software und Datenbank zur Ganzheitlichen
DIBt Bilanzierung, Professional Datenbank, Content Version
Deutsches Institut für Bautechnik 2021.2, Service Pack 40. LBP, Universität Stuttgart
und thinkstep, 2021.
ECHA Kandidatenliste Dokumentation der Datensätze unter
Liste der für eine Zulassung in Frage kommenden http://www.gabisoftware. com/deutsch/my-
besonders besorgniserregenden Stoffe (Stand: 07/22) gabi/gabidocumentation/.
gemäß Artikel 59 Absatz 10 der REACH-Verordnung.
European Chemicals Agency. IBU 2021
Institut Bauen und Umwelt e.V.: General Instructions
EN 318 for the EPD programme of Institut Bauen und Umwelt
Wood-based panels - Determination of dimensional e.V., Version 2.0, Berlin: Institut Bauen und Umwelt
changes associated with changes in relative humidity; e.V., 2021 www.ibu-epd.com
German version EN 318:2002
ISO 9001
EN 319 DIN EN ISO 9001:2015-11,
Particleboards and fibreboards; determination of Qualitätsmanagementsysteme - Anforderungen
tensile strength perpendicular to the plane of the (ISO 9001:2015); Deutsche und Englische Fassung
board; German version EN 319:1993 EN ISO 9001:2015
EN 12467 ISO 10456
8 Environmental Product Declaration Knauf AQUAPANEL GmbH & Co. KG – AQUAPANEL® Cement Board Outdoor - Site
Volos
DIN EN ISO 10456:2010-05,Building materials and concerning the Registration, Evaluation, Authorisation
products - Hygrothermal properties - Tabulated design and Restriction of Chemicals (REACH), establishing a
values and procedures for determining declared and European Chemicals Agency, amending Directive
design thermal values (ISO 10456:2007 + Cor.1:2009). 1999/45/EC and repealing Council Regulation (EEC)
No 793/93 and Council Regulation (EC) No
ISO 12572 1488/2006.
ISO 12572:2016-08,Hygrothermal performance of establishing a European Chemicals Agency, amending
building materials and products - Determination of Directive 1999/45/EC and repealing Council
water vapour transmission properties - Cup method Regulation (EEC) No 793/93 and Commission
Regulation (EC) No 1488/94 as well as Council
ISO 14025 Directive 76/769/EEC and Commission Directives
DIN EN ISO 14025:2011-10, Environmental labels and 91/155/EEC, 93/67/EEC, 93/105/EC and 2000/21/EC
declarations - Type III environmental declarations - (OJ L396, 30.12.2006, p. 1. Corrected version in OJ L
Principles and procedures 136, 29.5.2007, p. 3).
ISO 17294-2 Regulation (EU) No 305/2011
DIN EN ISO 17294-2:2017-01, Water quality - Regulation (EU) No 305/2011 of the European
Application of inductively coupled plasma mass Parliament and of the Council of 9 March 2011 laying
spectrometry (ICP-MS) - Part 2: Determination of down harmonised conditions for the marketing of
selected elements including uranium isotopes construction products and repealing Council Directive
89/106/EEC Text with EEA relevance.
Product Category Rules for Building-Related
Products and Services – Part A: Regulation (EU) No 528/2012
Product Category Rules for Building-Related Products Regulation (EU) No 528/2012 of the European
and Services. Part A: Calculation Rules for the Life Parliament and of the Council of 22 May 2012 1
Cycle Assessment and Requirements on the Project
Report, V2.1, 11/2021. Test report No. 3020-1166
Institute for Building Biology Rosenheim, Test report
PCR: Fibre Cement/Fibre Concrete Nr. 3020-1166 for AQUAPANEL® Cement Board
Product category rules for building-related products Indoor/Outdoor, 09-12-2020.
and services. Part B: Environmental Product
Declaration Requirements for Fibre Cement/Fibre Technical datasheet 08/17
Concrete. Berlin: Institut Bauen und Umwelt e.V. (ed.), Technical datasheet AQUAPANEL® Cement Board
01/2019. Outdoor, 08/17.
Regulation (EC) No 1907/2006
Regulation (EC) No 1907/2006 of the European
Parliament and of the Council of 18 December 2006
9 Environmental Product Declaration Knauf AQUAPANEL GmbH & Co. KG – AQUAPANEL® Cement Board Outdoor - Site
Volos
Publisher
Institut Bauen und Umwelt e.V. Tel +49 (0)30 3087748- 0
Hegelplatz 1 Fax +49 (0)30 3087748- 29
10117 Berlin Mail info@ibu-epd.com
Germany Web www.ibu-epd.com
Programme holder
Institut Bauen und Umwelt e.V. Tel +49 (0)30 - 3087748- 0
Hegelplatz 1 Fax +49 (0)30 – 3087748 - 29
10117 Berlin Mail info@ibu-epd.com
Germany Web www.ibu-epd.com
Author of the Life Cycle
Assessment Tel 02505 - 89-0
WESSLING GmbH Fax 02505 - 89 - 279
Oststraße 7 Mail info@wessling.de
48341 Altenberge Web www.wessling.de
Germany
Owner of the Declaration
Knauf AQUAPANEL GmbH & Co. Tel 0231 880855-0
KG Fax 0231 880855-31
Zur Helle 11 Mail aquapanel.info@knauf.com
58638 Iserlohn Web www.aquapanel.com
Germany
