ENVIRONMENTAL PRODUCT DECLARATION
as per ISO 14025 and EN 15804+A2
Owner of the Declaration dormakaba International Holding GmbH
Publisher Institut Bauen und Umwelt e.V. (IBU)
Programme holder Institut Bauen und Umwelt e.V. (IBU)
Declaration number EPD-DOR-20220206-CBA11-EN
Issue date 29.11.2022
Valid to 28.11.2027
Mortise Lock - DL Series 2xxx-9xxx
dormakaba
www.ibu-epd.com | https://epd-online.com
General Information
dormakaba Mortise Lock - DL Series 2xxx-9xxx
Programme holder Owner of the declaration
IBU – Institut Bauen und Umwelt e.V. dormakaba International Holding GmbH
Hegelplatz 1 DORMA Platz 1
10117 Berlin 58256 Ennepetal
Germany Germany
Declaration number Declared product / declared unit
EPD-DOR-20220206-CBA11-EN 1 Mortise Lock (1 piece) of the DL 9xxx Series, consisting of the following
items:
- one (1) mortise lock DL 91925
- one (1) closed case
- one (1) forend
- product packaging
This declaration is based on the product category rules: Scope:
Building Hardware products, 01.08.2021 This declaration is a specific product declaration for the Mortise Lock - DL
(PCR checked and approved by the SVR) Series 9xxx manufactured at production facility DKF7. The production site
is located in China. The underlying life cycle assessment is based on the
entire life cycle of this specific mortise lock series. The EPD is also
Issue date applicable for the Mortise Lock - DL Series 8xxx, 7xxx, 5xxx, 4xxx, 3xxx,
2xxx. Data represents the year 2022.
29.11.2022
The owner of the declaration shall be liable for the underlying information
and evidence; the IBU shall not be liable with respect to manufacturer
information, life cycle assessment data and evidences.
Valid to
28.11.2027 The EPD was created according to the specifications of EN 15804+A2. In
the following, the standard will be simplified as EN 15804.
Verification
The standard EN 15804 serves as the core PCR
Independent verification of the declaration and data according to ISO
14025:2011
internally X externally
Dipl.-Ing. Hans Peters
(Chairman of Institut Bauen und Umwelt e.V.)
Florian Pronold Dr.-Ing. Wolfram Trinius,
(Managing Director Institut Bauen und Umwelt e.V.) (Independent verifier)
1 Environmental Product Declaration - dormakaba - Mortise Lock - DL Series 2xxx-9xxx
Product
The DL Series 2xxx-5xxx has below technical properties:
Product description/Product definition
dormakaba Mortise Lock - DL Series 2xxx-9xxx for timber and
steel doors. DL Series locks are a complementary series of the
SIS size locks.
A range of mechanically operated locks for doors in buildings.
A complete range of high-quality products and functional
reliablity.
With the use of high-grade materials, precise production
techniques and a comprehensive quality management system,
all dormakaba locks meet demanding technical specifications.
Locks are supplied complete with fixing screws.
For the use and application of the product the respective
Performance data of the product with respect to its
national provisions at the place of use apply.
characteristics in accordance with the relevant technical
dormakaba locks are subject to strict quality requirements and
provision which can be applied are mentioned above.
are tested and certified according to:
Base materials/Ancillary materials
• EN 12209
The material composition of the Mortise lock - DL Series 9xxx is
the following:
Application
dormakaba DL locks Series locks can be used universally on
standard doors by changing the latch handing. Moreover they
offer their precision by a simple, compatible assembling in
standard door cuts.
As well as for applications with increased security
requirements.
dormakaba DL Series locks are as well fire-tested and RISE-
approved.
Technical Data
The Mortise Lock - DL Series 8xxx-9xxx fullfils following
technical properties:
The product includes partial articles which contain substances
listed in the Candidate List of REACH Regulation 1907/2006 /
EC (date: 14.06.2023) exceeding 0.1 percent by mass: no.
The Candidate List can be found on the ECHA website
address:
The following technical data are applicable for DL Series 7xxx: https: echa.europa.eu/de/home.
Reference service life
dormakaba Mortise Lock - DL Series 2xxx-9xxx is certified
according to EN 12209 up to 200.000 cycles of use. Under
normal conditions and depending on cycle frequency, door
weight and environmental conditions a duration of 15 years can
be secured.
LCA: Calculation rules
The type of EPD is according to EN 15804: "cradle to
Declared Unit gate with options, modules C1–C4, and module D".
The declared unit is 1 piece of the product: Mortise Lock - DL The following modules are declared: A1-A3, C1-C4, D
9xxx Series and additional modules: A4 + A5
Name Value Unit
Declared unit 1 piece/product Production - Module A1-A3
The product stage includes:
Mass of declared Product 0.769 kg
— A1, raw material extraction, processing and
mechanical treatments, processing of secondary
System boundary
material input (e.g. recycling processes),
2 Environmental Product Declaration - dormakaba - Mortise Lock - DL Series 2xxx-9xxx
— A2, transport to the manufacturer, including provision and all transport, provision of all
— A3, manufacturing and assembly materials, products and related energy and water use.
including provision of all materials, products and energy, as well Module D (Benefits and loads beyond the system
as waste processing up to the end-of waste state. boundary) includes:
— D, recycling potentials, expressed as net impacts
Construction stage - Modules A4-A5 and benefits.
The construction process stage includes:
— A4, transport to the building site; Geographic Representativeness
— A5, installation into the building; Land or region, in which the declared product system is
including provision of all materials, products and energy, as well manufactured, used or handled at the end of the product´s
as waste processing up to the end-of waste state or disposal of lifespan: Europe
final residues during the construction process stage.
Comparability
End-of-life stage– Modules C1-C4 and D
Basically, a comparison or an evaluation of EPD data is only
The end-of-life stage includes:
possible if all the data sets to be compared were created
— C1, de-construction, demolition:
according to EN 15804 and the building context, respectively
— C2, transport to waste processing;
the product-specific characteristics of performance, are taken
— C3, waste processing for reuse, recovery and/or
into account.
recycling;
— C4, disposal;
LCA: Scenarios and additional technical information
Reference service life
Characteristic product properties of biogenic carbon
Name Value Unit
Information on describing the biogenic Carbon Content at
Life Span according to the manufacturer 15 a
factory gate
Name ValueUnit End of life (C1-C4)
Biogenic carbon content in accompanying kg C1: The product dismantling from the building is done manually
0.006
packaging C without environmental burden.
Name Value Unit
Additional technical information for the Collected separately waste type 0.753 kg
declared modules. Recycling 0.752 kg
Transport to the building site (A4) Energy recovery 0.0006 kg
Name Value Unit Landfilling - kg
Litres of fuel (per 1kg) 0.00276l/100km
The product is disassembled in a recycling process.
Transport distance via truck (from habor to Material recycling is then assumed for the metals.
300 km
dormakaba logistic centre) The plastic components are assumed to be incinerated with
Capacity utilisation (including empty runs) 55 % energy recovery.
Transport distance via truck (for scaling) 100 km Region for the End of Life is: EU.
Transport distance via ship 13.000 km
Reuse, recovery and/or recycling potentials (D), relevant
The product is transported via truck and ship. The product is
scenario information
stored in the dormakaba logistic centre in Sweden. The main
Name Value Unit
distribution region is Scandinavia and the Baltic States with the
calculated transport distances. In order to allow scaling to a The collection rate is 100 %.
specific point of installation 100 km is declared as well.
Installation into the building (A5)
Name Value Unit
Waste packaging (paper) 0.01552 kg
Waste packaging (plastic) 0.0018 kg
3 Environmental Product Declaration - dormakaba - Mortise Lock - DL Series 2xxx-9xxx
LCA: Results
DESCRIPTION OF THE SYSTEM BOUNDARY (X = INCLUDED IN LCA; ND = MODULE OR INDICATOR NOT DECLARED; MNR =
MODULE NOT RELEVANT)
Benefits and
Construction loads beyond
Product stage Use stage End of life stage
process stage the system
boundaries
la ire ta m w a Ry lp p u s tro p s n a rT g n iru tc a fu n a M e h t m o rf tro p s n a rTe tis e h t o t e ta g y lb m e s s A e s U e c n a n e tn ia M ria p e R tn e m e c a lp e R tn e m h s ib ru fe R y g re n e la n o ita re p Oe s u re ta w la n o ita re p Oe s u n o itc u rts n o c -e Dn o itilo m e d tro p s n a rT g n is s e c o rp e ts a W la s o p s iD -e s u e R-y re v o c e R-g n ilc y c e Rla itn e to p
A1 A2 A3 A4 A5 B1 B2 B3 B4 B5 B6 B7 C1 C2 C3 C4 D
X X X X X MND MND MNR MNR MNR MND MND X X X X X
RESULTS OF THE LCA - ENVIRONMENTAL IMPACT according to EN 15804+A2: 1 piece Mortise Lock - DL Series 2xxx-9xxx
Parameter Unit A1-A3 A4 A5 C1 C2 C3 C4 D
GWP-total kg CO 2 eq 2.69E+00 6E-02 2.7E-02 0 3E-03 2E-03 0 -1.74E+00
GWP-fossil kg CO 2 eq 2.72E+00 5.8E-02 5E-03 0 3E-03 2E-03 0 -1.74E+00
GWP-biogenic kg CO 2 eq -2.69E-02 1E-03 2.1E-02 0 1.44E-04 3.55E-08 0 4E-03
GWP-luluc kg CO 2 eq 4.3E-03 1.29E-06 6.21E-07 0 7.43E-08 8.62E-08 0 -2E-03
ODP kg CFC11 eq 1.88E-13 5.81E-18 6.27E-18 0 3.29E-19 7.69E-19 0 -2.09E-15
AP mol H+ eq 1.18E-02 1E-03 6.98E-06 0 3.12E-06 2.72E-07 0 -7E-03
EP-freshwater kg P eq 5.04E-06 1.29E-08 1.14E-09 0 6.68E-10 1.23E-10 0 -1.98E-06
EP-marine kg N eq 2.18E-03 3.27E-04 2.41E-06 0 9.94E-07 6.12E-08 0 -1E-03
EP-terrestrial mol N eq 1.9E-02 4E-03 3.15E-05 0 1.11E-05 1.24E-06 0 -1.2E-02
kg NMVOC
POCP 5.52E-03 9.13E-04 6.41E-06 0 2.81E-06 1.69E-07 0 -4E-03
eq
ADPE kg Sb eq 4.7E-04 1.61E-09 9.43E-11 0 9.36E-11 1.06E-11 0 -1.79E-04
ADPF MJ 3.3E+01 7.61E-01 9E-03 0 4.4E-02 7.07E-04 0 -1.95E+01
m3 world eq
WDP 7.92E-01 1.09E-04 3E-03 0 6.12E-06 1.56E-04 0 -4.8E-01
deprived
GWP = Global warming potential; ODP = Depletion potential of the stratospheric ozone layer; AP = Acidification potential of land and water; EP =
Eutrophication potential; POCP = Formation potential of tropospheric ozone photochemical oxidants; ADPE = Abiotic depletion potential for non-fossil
resources; ADPF = Abiotic depletion potential for fossil resources; WDP = Water (user) deprivation potential)
RESULTS OF THE LCA - INDICATORS TO DESCRIBE RESOURCE USE according to EN 15804+A2: 1 piece Mortise Lock - DL
Series 2xxx-9xxx
Parameter Unit A1-A3 A4 A5 C1 C2 C3 C4 D
PERE MJ 8.48E+00 2E-03 1.88E-01 0 1.4E-04 1.84E-04 0 -3.18E+00
PERM MJ 1.86E-01 0 -1.86E-01 0 0 0 0 0
PERT MJ 8.67E+00 2E-03 2E-03 0 1.4E-04 1.84E-04 0 -3.18E+00
PENRE MJ 3.3E+01 7.62E-01 8.6E-02 0 4.4E-02 2.2E-02 0 -1.96E+01
PENRM MJ 9.8E-02 0 -7.7E-02 0 0 -2.1E-02 0 0
PENRT MJ 3.31E+01 7.62E-01 9E-03 0 4.4E-02 7.07E-04 0 -1.96E+01
SM kg 3.26E-01 0 0 0 0 0 0 0
RSF MJ 0 0 0 0 0 0 0 0
NRSF MJ 0 0 0 0 0 0 0 0
FW m3 2.8E-02 4.43E-06 7.54E-05 0 2.5E-07 3.73E-06 0 -1.9E-02
PERE = Use of renewable primary energy excluding renewable primary energy resources used as raw materials; PERM = Use of renewable primary
energy resources used as raw materials; PERT = Total use of renewable primary energy resources; PENRE = Use of non-renewable primary energy
excluding non-renewable primary energy resources used as raw materials; PENRM = Use of non-renewable primary energy resources used as raw
materials; PENRT = Total use of non-renewable primary energy resources; SM = Use of secondary material; RSF = Use of renewable secondary fuels;
NRSF = Use of non-renewable secondary fuels; FW = Use of net fresh water
RESULTS OF THE LCA – WASTE CATEGORIES AND OUTPUT FLOWS according to EN 15804+A2:
1 piece Mortise Lock - DL Series 2xxx-9xxx
Parameter Unit A1-A3 A4 A5 C1 C2 C3 C4 D
HWD kg 1.15E-07 7.44E-11 1.83E-11 0 4.3E-12 2.7E-12 0 -2.13E-07
NHWD kg 1.86E-01 7.8E-05 1E-03 0 4.53E-06 1.58E-04 0 -8.5E-02
RWD kg 1.19E-03 8.34E-07 4.44E-07 0 4.76E-08 2.62E-08 0 -2.44E-04
CRU kg 0 0 0 0 0 0 0 0
MFR kg 0 0 0 0 0 7.46E-01 0 0
MER kg 0 0 0 0 0 0 0 0
EEE MJ 6.86E-05 0 4.2E-02 0 0 0 0 0
EET MJ 1.25E-04 0 8E-02 0 0 0 0 0
4 Environmental Product Declaration - dormakaba - Mortise Lock - DL Series 2xxx-9xxx
HWD = Hazardous waste disposed; NHWD = Non-hazardous waste disposed; RWD = Radioactive waste disposed; CRU = Components for re-use;
MFR = Materials for recycling; MER = Materials for energy recovery; EEE = Exported electrical energy; EET = Exported thermal energy
RESULTS OF THE LCA – additional impact categories according to EN 15804+A2-optional:
1 piece Mortise Lock - DL Series 2xxx-9xxx
Parameter Unit A1-A3 A4 A5 C1 C2 C3 C4 D
Disease
PM 1.79E-07 2.07E-08 4.45E-11 0 1.64E-11 3.46E-12 0 -1.26E-07
incidence
IR kBq U235 eq 1.31E-01 1.2E-04 6.36E-05 0 6.79E-06 2.36E-06 0 -2.8E-02
ETP-fw CTUe 1.43E+01 5.39E-01 4E-03 0 3.1E-02 2.65E-04 0 -8.94E+00
HTP-c CTUh 3.21E-07 1.01E-11 2.43E-13 0 5.9E-13 2.3E-14 0 -1.23E-09
HTP-nc CTUh 8.76E-08 4.59E-10 1.45E-11 0 2.52E-11 2.33E-12 0 1.55E-07
SQP SQP 9.43E+00 2E-03 2E-03 0 1.14E-04 2.12E-04 0 -1.77E+00
PM = Potential incidence of disease due to PM emissions; IR = Potential Human exposure efficiency relative to U235; ETP-fw = Potential comparative
Toxic Unit for ecosystems; HTP-c = Potential comparative Toxic Unit for humans (cancerogenic); HTP-nc = Potential comparative Toxic Unit for humans
(not cancerogenic); SQP = Potential soil quality index
Disclaimer 1 – for the indicator “Potential Human exposure efficiency relative to U235”. This impact category deals mainly with the
eventual impact of low-dose ionizing radiation on human health of the nuclear fuel cycle. It does not consider effects due to possible
nuclear accidents, occupational exposure or radioactive waste disposal in underground facilities. Potential ionizing radiation from the
soil, radon and from some construction materials is also not measured by this indicator.
Disclaimer 2 – for the indicators “abiotic depletion potential for non-fossil resources”, “abiotic depletion potential for fossil resources”,
“water (user) deprivation potential, deprivation-weighted water consumption”, “potential comparative toxic unit for ecosystems”,
“potential comparative toxic unit for humans – cancerogenic”, “Potential comparative toxic unit for humans - not cancerogenic”,
“potential soil quality index”. The results of this environmental impact indicator shall be used with care as the uncertainties on these
results are high as there is limited experience with the indicator.
References
EN 12209 Sphera Solutions GmbH
EN 12209:2003 Building hardware – locks and latches – Gabi Software System and Database for Life Cycle
mechanically operated locks, latches and locking plates – Engineering 1992-2020
requirements and methods Version 10.0.0.71
University of Stuttgart
EN 15804 Leinfelden-Echterdingen
EN 15804+A2:2019+AC:2021, Sustainability of construction
works — Environmental Product Declarations — Core rules for GaBi ts documentation
the product category of construction products. GaBi life cycle inventory data documentation (https://www.gabi-
software.com/support/gabi/gabidatabase- 2020-lci-
ISO 14025 documentation/).
DIN EN ISO 14025:201110, Environmental labels and
declarations — Type III environmental declarations — LCA-tool dormakaba
Principles and procedures. LCA tool DHW. LCA-Tool No.: IBU-DOR-202104-LT1-EN.
Developed by Sphera Solutions GmbH
REACH
Regulation (EC) No 1907/2006 of the European Parliament and PCR Part A
of the Council on the Registration, Evaluation, Authorisation PCR – Part A: Calculation Rules for the Life Cycle Assessment
and Restriction of Chemicals (REACH) and Requirements on the Project Re-port
according to EN 15804+A2:2019, Version 1.0, 2020, Institut
Further References Bauen und Umwelt e.V., www.ibu-epd.com.
IBU 2021 PCR Part B
General Instructions for the EPD programme of Institut Bauen PCR – Part B: Requirements on the EPD for Building Hardware
und Umwelt e.V. ; Version 2.0, Berlin: Institut product, version 08/2021, Institut Bauen und Umwelt e.V.,
Bauen und Umwelt e.V., 2021. www.ibu-epd.com www.ibu-epd.com.
GaBi
5 Environmental Product Declaration - dormakaba - Mortise Lock - DL Series 2xxx-9xxx
Publisher
Institut Bauen und Umwelt e.V. +49 (0)30 3087748- 0
Hegelplatz 1 info@ibu-epd.com
10117 Berlin www.ibu-epd.com
Germany
Programme holder
Institut Bauen und Umwelt e.V. +49 (0)30 3087748- 0
Hegelplatz 1 info@ibu-epd.com
10117 Berlin www.ibu-epd.com
Germany
Author of the Life Cycle Assessment
Sphera Solutions GmbH +49 711 341817-0
Hauptstraße 111- 113 info@sphera.com
70771 Leinfelden-Echterdingen www.sphera.com
Germany
Owner of the Declaration
dormakaba International Holding GmbH +49 2333 793-0
DORMA Platz 1 info.de@dormakaba.com
58256 Ennepetal www.dormakaba.com
Germany
6 Environmental Product Declaration - dormakaba - Mortise Lock - DL Series 2xxx-9xxx
