ENVIRONMENTAL PRODUCT DECLARATION
as per ISO 14025 and EN 15804+A2
Owner of the Declaration Kingspan Insulation B.V.
Publisher Institut Bauen und Umwelt e.V. (IBU)
Programme holder Institut Bauen und Umwelt e.V. (IBU)
Declaration number EPD-KSI-20230167-CBA1-EN
Issue date 11.07.2023
Valid to 10.07.2028
Kooltherm® K8 D Plus
Kingspan Insulation B.V.
www.ibu-epd.com | https://epd-online.com
General Information
Kingspan Insulation B.V. Kooltherm® K8 D Plus
Programme holder Owner of the declaration
IBU – Institut Bauen und Umwelt e.V. Kingspan Insulation B.V.
Hegelplatz 1 Lingewei 8
10117 Berlin 4004LL Tiel
Germany Netherlands
Declaration number Declared product / declared unit
EPD-KSI-20230167-CBA1-EN Kooltherm® K8 D Plus Cavity Wall Board 1 m², 120 mm thickness (100mm
Kooltherm + 20mm mineral wool) R = 5,35 m²·K/W
D
This declaration is based on the product category rules: Scope:
Insulating materials made of foam plastics, 01.08.2021 The insulation material Kooltherm® is produced by Kingspan Insulation
(PCR checked and approved by the SVR) B.V. at the manufacturing facility in Tiel, the Netherlands. A composite foil
based facing is autohesively bonded to the insulation core during
manufacture. On the backside a 20mm mineral wool layer is bonded
Issue date afterwards.
In order to enable the user of the EPD to calculate the LCA results for
11.07.2023
different thicknesses, the EPD contains the respective calculation rules.
The owner of the declaration shall be liable for the underlying information
and evidence; the IBU shall not be liable with respect to manufacturer
Valid to
information, life cycle assessment data and evidences.
10.07.2028
The EPD was created according to the specifications of EN 15804+A2. In
the following, the standard will be simplified as EN 15804.
Verification
The standard EN 15804 serves as the core PCR
Independent verification of the declaration and data according to ISO
14025:2011
internally X externally
Dipl.-Ing. Hans Peters
(Chairman of Institut Bauen und Umwelt e.V.)
Florian Pronold Vito D'Incognito,
(Managing Director Institut Bauen und Umwelt e.V.) (Independent verifier)
1 Environmental Product Declaration - Kingspan Insulation B.V. - Kooltherm® K8 D Plus
Product
Technical parameters not included are modulus of elasticity as
Product description/Product definition well as sound absorption (not relevant for this application), and
Kooltherm® K8 D Plus is a rigid thermoset cellular insulation creep (not placed under permanent load).
material faced on both sides with a composite foil based facing.
On the backside a mineral wool (20 mm) is bonded. The Performance data of the product in accordance with the
product is available in variable thicknesses from 40 mm (20+20 declaration of performance with respect to its essential
mm) up to 220 mm (200+20 mm). This EPD covers one of the characteristics according to EN 13166:2012+A2:2016 - Thermal
most commonly sold thickness of 120 mm (100+20 mm) with insulation products for buildings - Factory made phenolic foam
an R D-value of 5,35 m²·K/W. (PF) products - Specification
Base materials/Ancillary materials
For the placing on the market of the product in the European
Union/European Free Trade Association (EU/EFTA) (with the The main materials are phenolic (PF) resin (between 70-80%)
exception of Switzerland) Regulation (EU) No. 305/2011 (CPR) with added catalyst and additives (between 15-20%). Phenolic
applies. The product needs a declaration of performance taking rigid foam onto a facing material (between 5-10%) is formed by
into consideration EN 13166:2012+A2:2016 - Thermal the chemical reaction of these materials and adding a blowing
insulation products for buildings - Factory made phenolic foam agent with no ozone depletion potential (ca. 5%). Due to the
(PF) products - Specification and the CE-marking. For the closed-cell structure (conform EN 13166), the blowing agent
application and use the respective national provisions apply. remains in the foam. In the current REACH regulations,
phenolic foam insulation products are considered 'articles' and
Application are exempt from the requirements of Article 57 and 59(1) of
Due to its high insulating value, Kooltherm® K8 D Plus is REACH Regulation (EC) No 1907/2006. These products are
suitable for use as cavity wall insulation. The extra layer mineral not classified as 'hazardous products' according to any current
wool (20 mm) will absorb unevenness in a construction, which legislation, and can hence be declared as follows:
makes Kooltherm® K8 D Plus suitable for renovation projects. - This article contains substances listed in the candidate list
(date: 19.01.2021) exceeding 0.1 percentage by mass: no.
Technical Data - This article contains other carcinogenic, mutagenic, reprotoxic
(CMR) substances in categories 1A or 1B which are not on the
Constructional data
candidate list, exceeding 0.1 percentage by mass: no.
Name Value Unit
- Biocide products were added to this construction product or it
Compressive strength acc. to EN 13166 ≥ 100 kPa has been treated with biocide products (this then concerns a
Thermal conductivity λd acc. to EN 13166 for d treated product as defined by the (EU) Biocidal Products
0.021W/(mK)
= 20 – 44 mm Regulation No. 528/2012 (BPR): no.
Thermal conductivity λd acc. to EN 13166 for d
= 45 – 120 mm 0.021W/(mK) The chemical functional group of the additives used in the resin
is that of non-ionic surfactants.
Thermal conductivity λd acc. to EN 13166 for d
0.021W/(mK)
= 121 – 159 mm Reference service life
Thermal conductivity λd (mineral wool) acc. to 0.034W/(mK) The reference service life is not to be declared in this EPD as it
EN 13162 for d = 20 mm does not cover the use stage.
LCA: Calculation rules
processing of secondary material input (e.g. recycling
Declared Unit processes),
The declared unit (1 m²) and conversion factors are listed in the · A2, transport to the manufacturer,
table below. · A3, manufacturing,
Declared unit including provision of all materials, products and
energy, packaging processing and its transport, as well
Name Value Unit
as waste processing up to the end-of-waste state or
Declared unit thickness 120 mm (100+20 mm) 1 m2 disposal of final residues during the product stage.
Gross density 34.1 kg/m3
conversion factor [Mass/Declared Unit] ( in kg/m² )4.092 - The construction process stage includes:
· A4 transport to the building site;
Grammage 4.092kg/m2
· A5 installation in the building
Layer thickness 0.12 m including provision of all materials, products and energy, as well
as waste processing up to the end-of-waste state or disposal of
System boundary final residues during the construction process stage.
Type of EPD: according to EN 15804:
cradle to gate with options, modules C1–C4, and module D The end-of-life stage is a mandatory information module and it
(A1–A3, C, D and additional modules: A4,A5). covers:
According to PCR Part A: · C1 de-construction, demolition;
1a) declaration of one specific product from one plant · C2 transport to waste processing;
of one manufacturer; · C3 waste processing for reuse, recovery and/or recycling;
· C4 disposal (not applicable for this EPD)
The product stage is a mandatory information module including provision and all transport, provision of all materials,
and it covers: products and related energy and water use.
· A1, raw material extraction and processing,
2 Environmental Product Declaration - Kingspan Insulation B.V. - Kooltherm® K8 D Plus
Environmental burden of the incineration (R1 > 60%) of the
product at the end-of-life stage are assigned to the product Background database
system (C3); resulting potential credits for thermal and electrical Background data from GaBi software-system version 9 with
energy from energy substitution are declared in module D. Service Packs 39 GaBi ts is used.
Renewable electricity sources for manufacturing Geographic Representativeness
All electricity used during production comes from renewable Land or region, in which the declared product system is
sources. manufactured, used or handled at the end of the product´s
By generating energy on-site with solar panels and with lifespan: Europe
procured energy from fully certified renewable sources.
Following the global Net Zero Energy strategy from Kingspan
Comparability
Group plc.
Basically, a comparison or an evaluation of EPD data is only
possible if all the data sets to be compared were created
Period under review
according to EN 15804 and the building context, respectively
The input data for raw material production and the consumption
the product-specific characteristics of performance, are taken
of process energy on the manufacturing facility was measure
into account.
data during January 1st 2019 to December 31st 2019, i.e.
collected over a 12 month period.
LCA: Scenarios and additional technical information
conditions underlying the determined RSL shall be declared. In
Characteristic product properties of biogenic carbon addition, it shall be stated that the RSL applies to the reference
The total mass of biogenic carbon containing materials is less conditions only.
than 5 % of the total mass of the product and accompanying
packaging. The same holds for a service life declared by the manufacturer.
Technical information Corresponding information related to in-use conditions needs
The following technical information is a basis for the declared not be provided if a service life taken from the list of service life
modules or can be used for developing specific scenarios in the by BNB is declared.
context of a building assessment.
Transport to the building site (A4) End of life (C1-C4)
Name Value Unit The assumptions for C1 are: diesel driven excavator (100 kW;
Litres of fuel 0.0103 l/100km 0.2 litre fuel per ton excavated material).
The assumptions for C2 are: Truck Euro 6, diesel driven, 26-28
Transport distance 100 km
t gross weight, assumed distance 50 km
Gross density of products transported 34.1 kg/m3
Name Value Unit
Installation into the building (A5) Collected as mixed construction waste 4.09 kg
Name ValueUnit Energy recovery 4.09 kg
Output substances following waste treatment on R1-value of waste incineration plant >60 %
0.08 kg
site packaging material
Reuse, recovery and/or recycling potentials (D),
Within A1-A3 the following packaging of the final product is relevant scenario information
included:
Polyethylene cover and wrap: 0,06 kg/m² Waste incineration with energy recuperation is
Others (mainly Expanded Polystyrene skid): 0,02 kg/m² assumed as end-of-life scenario
The recycling of the packaging is considered in A5.
In case a reference service life according to applicable ISO
standards is declared then the assumptions and in-use
3 Environmental Product Declaration - Kingspan Insulation B.V. - Kooltherm® K8 D Plus
LCA: Results
Disclaimer:
EP-freshwater: This indicator has been calculated as “kg P eq” as required in
the characterization model (EUTREND model, Struijs et al., 2009b, as
implemented in ReCiPe; http://eplca.jrc.ec.europa.eu/LCDN/developerEF.xhtml)
DESCRIPTION OF THE SYSTEM BOUNDARY (X = INCLUDED IN LCA; ND = MODULE OR INDICATOR NOT DECLARED; MNR =
MODULE NOT RELEVANT)
Benefits and
Construction loads beyond
Product stage Use stage End-of-life stage
process stage the system
boundaries
la ire ta m w a Ry lp p u s tro p s n a rT g n iru tc a fu n a M e h t m o rf tro p s n a rTe tis e h t o t e ta g y lb m e s s A e s U e c n a n e tn ia M ria p e R tn e m e c a lp e R tn e m h s ib ru fe R y g re n e la n o ita re p Oe s u re ta w la n o ita re p Oe s u n o itc u rts n o c -e Dn o itilo m e d tro p s n a rT g n is s e c o rp e ts a W la s o p s iD -e s u e R-y re v o c e R-g n ilc y c e Rla itn e to p
A1 A2 A3 A4 A5 B1 B2 B3 B4 B5 B6 B7 C1 C2 C3 C4 D
X X X X X MND MND MNR MNR MNR MND MND X X X X X
RESULTS OF THE LCA - ENVIRONMENTAL IMPACT according to EN 15804+A2: 1 m2 120 mm thickness (100+20 mm)
Parameter Unit A1-A3 A4 A5 C1 C2 C3 C4 D
GWP-total kg CO 2 eq 8.75E+00 3.51E-02 2E-01 2.64E-03 1.75E-02 8.29E+00 0 -3.55E+00
GWP-fossil kg CO 2 eq 8.9E+00 3.47E-02 2E-01 2.64E-03 1.74E-02 8.29E+00 0 -3.54E+00
GWP-biogenic kg CO 2 eq -2.28E-01 -2.11E-04 -3.63E-06 -1.86E-07 -1.06E-04 8.57E-04 0 -6.87E-03
GWP-luluc kg CO 2 eq 7.95E-02 5.31E-04 7.2E-06 8.97E-08 2.66E-04 1.19E-04 0 -2.41E-03
ODP kg CFC11 eq 1.31E-08 4.22E-18 5.97E-17 2.54E-19 2.11E-18 1.14E-15 0 -3.62E-14
AP mol H+ eq 2.7E-02 4.1E-05 2.76E-05 1.26E-05 2.05E-05 4.76E-03 0 -6.69E-03
EP-freshwater kg P eq 2.83E-05 1.68E-07 1.05E-08 4.7E-10 8.38E-08 2.92E-07 0 -4.66E-06
EP-marine kg N eq 5.93E-03 1.26E-05 7.28E-06 5.87E-06 6.32E-06 2.26E-03 0 -1.54E-03
EP-terrestrial mol N eq 7.84E-02 1.48E-04 1.2E-04 6.43E-05 7.41E-05 2.61E-02 0 -1.65E-02
kg NMVOC
POCP 2.27E-02 3.3E-05 2.09E-05 1.67E-05 1.65E-05 5.82E-03 0 -4.41E-03
eq
ADPE kg Sb eq 6.56E-06 2.42E-09 8.6E-10 6.96E-11 1.21E-09 1.93E-08 0 -5.53E-07
ADPF MJ 2.22E+02 4.63E-01 7.91E-02 3.59E-02 2.31E-01 2.45E+00 0 -6.14E+01
m3 world eq
WDP 1.49E+00 7.49E-04 2.08E-02 4.62E-06 3.75E-04 8.54E-01 0 -3.29E-01
deprived
GWP = Global warming potential; ODP = Depletion potential of the stratospheric ozone layer; AP = Acidification potential of land and water; EP =
Eutrophication potential; POCP = Formation potential of tropospheric ozone photochemical oxidants; ADPE = Abiotic depletion potential for non-fossil
resources; ADPF = Abiotic depletion potential for fossil resources; WDP = Water (user) deprivation potential)
RESULTS OF THE LCA - INDICATORS TO DESCRIBE RESOURCE USE according to EN 15804+A2: 1 m2 120 mm thickness
(100+20 mm)
Parameter Unit A1-A3 A4 A5 C1 C2 C3 C4 D
PERE MJ 3.85E+01 2.69E-02 1.53E-02 1.05E-04 1.34E-02 3.42E-01 0 -1.24E+01
PERM MJ 0 0 0 0 0 0 0 0
PERT MJ 3.85E+01 2.69E-02 1.53E-02 1.05E-04 1.34E-02 3.42E-01 0 -1.24E+01
PENRE MJ 1.25E+02 4.63E-01 7.92E-02 3.59E-02 2.32E-01 1E+02 0 -6.14E+01
PENRM MJ 9.76E+01 0 0 0 0 -9.76E+01 0 0
PENRT MJ 2.22E+02 4.63E-01 7.92E-02 3.59E-02 2.32E-01 2.45E+00 0 -6.14E+01
SM kg 0 0 0 0 0 0 0 0
RSF MJ 0 0 0 0 0 0 0 0
NRSF MJ 0 0 0 0 0 0 0 0
FW m3 6.32E-02 4.54E-05 4.94E-04 1.95E-07 2.27E-05 2.02E-02 0 -1.46E-02
PERE = Use of renewable primary energy excluding renewable primary energy resources used as raw materials; PERM = Use of renewable primary
energy resources used as raw materials; PERT = Total use of renewable primary energy resources; PENRE = Use of non-renewable primary energy
excluding non-renewable primary energy resources used as raw materials; PENRM = Use of non-renewable primary energy resources used as raw
materials; PENRT = Total use of non-renewable primary energy resources; SM = Use of secondary material; RSF = Use of renewable secondary fuels;
NRSF = Use of non-renewable secondary fuels; FW = Use of net fresh water
RESULTS OF THE LCA – WASTE CATEGORIES AND OUTPUT FLOWS according to EN 15804+A2:
1 m2 120 mm thickness (100+20 mm)
Parameter Unit A1-A3 A4 A5 C1 C2 C3 C4 D
HWD kg 8.87E-05 2.59E-08 3.71E-10 3.8E-12 1.29E-08 4.89E-09 0 -2.52E-08
NHWD kg 3.73E-01 3.77E-05 1.93E-02 2.14E-07 1.88E-05 2.42E-01 0 -2.65E-02
RWD kg 3.54E-03 6.29E-07 3.64E-06 4.13E-08 3.14E-07 1.12E-04 0 -4.95E-03
CRU kg 0 0 0 0 0 0 0 0
4 Environmental Product Declaration - Kingspan Insulation B.V. - Kooltherm® K8 D Plus
MFR kg 0 0 0 0 0 0 0 0
MER kg 0 0 7.99E-02 0 0 4.09E+00 0 0
EEE MJ 0 0 4.43E-01 0 0 1.43E+01 0 0
EET MJ 0 0 7.98E-01 0 0 2.56E+01 0 0
HWD = Hazardous waste disposed; NHWD = Non-hazardous waste disposed; RWD = Radioactive waste disposed; CRU = Components for re-use;
MFR = Materials for recycling; MER = Materials for energy recovery; EEE = Exported electrical energy; EET = Exported thermal energy
RESULTS OF THE LCA – additional impact categories according to EN 15804+A2-optional:
1 m2 120 mm thickness (100+20 mm)
Parameter Unit A1-A3 A4 A5 C1 C2 C3 C4 D
Disease
PM 2.64E-07 2.36E-10 3.77E-10 1.41E-10 1.18E-10 1.64E-08 0 -5.67E-08
incidence
IR kBq U235 eq 5.84E-01 9.21E-05 4.82E-04 6.03E-06 4.6E-05 1.73E-02 0 -8.13E-01
ETP-fw CTUe 1.28E+02 3.12E-01 5.6E-02 2.42E-02 1.56E-01 9.55E-01 0 -1.36E+01
HTP-c CTUh 8.91E-09 6.26E-12 4.28E-12 4.12E-13 3.13E-12 1.35E-10 0 -2.5E-09
HTP-nc CTUh 1.15E-07 2.52E-10 3.14E-10 1.44E-11 1.26E-10 1.95E-09 0 -1.26E-08
SQP SQP 4.66E+01 2.09E-01 1.99E-02 9.39E-05 1.04E-01 5.16E-01 0 -9.23E+00
PM = Potential incidence of disease due to PM emissions; IR = Potential Human exposure efficiency relative to U235; ETP-fw = Potential comparative
Toxic Unit for ecosystems; HTP-c = Potential comparative Toxic Unit for humans (cancerogenic); HTP-nc = Potential comparative Toxic Unit for humans
(not cancerogenic); SQP = Potential soil quality index
Disclaimer 1 – for the indicator IR
This impact category deals mainly with the eventual impact of low dose ionizing radiation on human health of the nuclear fuel cycle. It
does not consider effects due to possible nuclear accidents, occupational exposure nor due to radioactive waste disposal in
underground facilities. Potential ionizing radiation from the soil, from radon and from some construction materials is also not measured
by this indicator.
Disclaimer 2 – for the indicators ADPE, ADPF, WDP, ETP-fw, HTP-c, HTP-nc, SQP
The results of this environmental impact indicator shall be used with care as the uncertainties on these results are high or as there is
limited experienced with the indicator.
Factors for different thicknesses
The LCA results for the insulation material declared in this EPD refer to a product with a thickness of 120 mm (100+20 mm). To enable
the user of the EPD to calculate the results for different thicknesses the factors in the following table can be used for the calculation.
For modules A1- A3, C3 and D the LCA results in chapter 5 have to be multiplied with these factors. As the 20 mm mineral wool layer is
for all products equal, it is the Kooltherm insulation foam that is scaling up- and downwards in thickness and is responsible for the
different scaling factors.
This EPD was created using a software tool.
References
EN13162
EN 13162:2012+A1:2015: Thermal insulation products for BPR
buildings. Factory made mineral wool (MW) products. Regulation (EU) No 528/2012 of the European Parliament and
Specification of the Council of 22 May 2012 concerning the making available
on the market and use of biocidal products
EN 13166
EN 13166:2012+A2:2016: Thermal insulation products for CPR
buildings. Factory made phenolic foam (PF) products. Regulation (EU) No. 305/2011 of the European Parliament and
Specification of the Council of 9 March 2011 laying down hamonised
condition for the marketing of construction products and
EN 15804+A2 repealing Council Directive 89/106/EC
EN15804/A2: Sustainability of construction works -
Environmental product declarations - Core rules for the product GaBi ts
category of construction products, 2019 thinkstep AG: Leinfelden-Echterdingen GaBi Software- System
5 Environmental Product Declaration - Kingspan Insulation B.V. - Kooltherm® K8 D Plus
and Database for Life Cycle Engineering 1992- 2019 Calculation Rules for the Life Cycle Assessment and
Requirements on the Project Report , March 2018
IBU 2016
IBU (2016): General Programme Instructions for the PCR 2017, Part B
Preparation of EPDs at the Institut Bauen und Umwelt e.V., Institut Bauen und Umwelt e.V., Berlin (pub.): Product Category
Version 1.1 Institut Bauen und Umwelt e.V., Berlin, www.ibu- Rules for Construction Products from the range of
epd.de Environmental Product Declarations of Institut Bauen und
Umwelt (IBU), Part B: Requirements on the EPD for insulating
ISO 14025 materials made of foam plastics.June 2017
EN ISO 14025:2011-10 - Environmental labels and declarations
— Type III environmental declarations — Principles and REACH
procedures Regulation (EC) No 1907/2006 of the European Parliament and
of the Council on the Registration, Evaluation, Authorisation
LCA-tool and Restriction of Chemicals (REACH)
Kingspan LCA tool, version 1.0. IBU-KSI-202001-LT1-EN. https://echa.europa.eu/candidate-list-table; accessed 19th of
Developed by Sphera Solutions GmbH (formely Thinkstep January 2021, 211 substances listed.
GmbH)
Renewable Energy Certificate
PCR Version 1.7, Part A Towarowa Gielda Energii S.A.: Guarantees of origin Document
Institut Bauen und Umwelt e.V., Berlin (pub.): Product Category ID: RGP_ACTBV_2019-12-31_0720
Rules for Building-Related Products and services, Part A:
6 Environmental Product Declaration - Kingspan Insulation B.V. - Kooltherm® K8 D Plus
Publisher
Institut Bauen und Umwelt e.V. +49 (0)30 3087748- 0
Hegelplatz 1 info@ibu-epd.com
10117 Berlin www.ibu-epd.com
Germany
Programme holder
Institut Bauen und Umwelt e.V. +49 (0)30 3087748- 0
Hegelplatz 1 info@ibu-epd.com
10117 Berlin www.ibu-epd.com
Germany
Author of the Life Cycle Assessment
Kingspan Insulation B.V. +31 (0) 543 543 210
Lingewei 8 info@kingspaninsulation.nl
4004LL Tiel www.kingspan.com
Netherlands
Owner of the Declaration
Kingspan Insulation B.V. +31 (0) 543 543 210
Lingewei 8 info@kingspaninsulation.nl
4004LL Tiel www.kingspan.com
Netherlands
7 Environmental Product Declaration - Kingspan Insulation B.V. - Kooltherm® K8 D Plus
