ENVIRONMENTAL PRODUCT DECLARATION
as per ISO 14025 and EN 15804+A2
Owner of the Declaration DuPont de Nemours (Luxembourg) s.à r.l.
Programme holder Institut Bauen und Umwelt e.V. (IBU)
Publisher Institut Bauen und Umwelt e.V. (IBU)
Declaration number EPD-DUP-20210183-IBC1-EN
Issue date 30.11.2021
Valid to 29.11.2026
DuPont™ Tyvek® Monolayer 60 (1060B, 1560B, 2460B)
DuPont de Nemours (Luxembourg) s.à r.l.
www.ibu-epd.com | https://epd-online.com
Umwelt Produktdeklaration Name des Herstellers – Name des Produkts
1. General Information
DuPont de Nemours (Luxembourg) s.à r.l. DuPont™ Tyvek® Monolayer 60
(1060B, 1560B, 2460B)
Programme holder Owner of the declaration
IBU – Institut Bauen und Umwelt e.V. DuPont de Nemours (Luxembourg) s.à r.l.
Panoramastr. 1 Rue Général Patton
10178 Berlin L-2984 Contern
Germany Luxembourg
Declaration number Declared product / declared unit
EPD-DUP-20210183-IBC1-EN 1 m² DuPont™ Tyvek® Monolayer (1060B, 1560B,
2460B)
This declaration is based on the product Scope:
category rules: This document applies to DuPont™ Tyvek® 1060B,
False ceiling and underlay sheeting, 11.2017 1560B and 2460B monolayer high density polyethylene
(PCR checked and approved by the SVR) (HDPE) membranes manufactured by DuPont in L-
2984 Contern and printed in Germany, with a declared
unit weight of 58 g/m2. The LCA data were compiled
Issue date
using production data from the year 2019 by DuPont
30.11.2021
Luxembourg s.à r.l. The declaration holder is
responsible for the underlying data and its verification.
Valid to
29.11.2026
The owner of the declaration shall be liable for the
underlying information and evidence; the IBU shall not
be liable with respect to manufacturer information, life
cycle assessment data and evidences.
The EPD was created according to the specifications
of EN 15804+A2. In the following, the standard will be
simplified as EN 15804.
Verification
The standard EN 15804 serves as the core PCR
Independent verification of the declaration and data
according to ISO 14025:2010
Dipl. Ing. Hans Peters internally x externally
(chairman of Institut Bauen und Umwelt e.V.)
Dr. Alexander Röder Vito D'Incognito
(Managing Director Institut Bauen und Umwelt e.V.)) (Independent verifier)
2. Product
2.1 Information about the enterprise and EN 13859-2:2010 : Flexible sheets for
DuPont is a global innovation leader with technology- waterproofing - Definitions and characteristics of
based materials and solutions that help transform underlays - Part 2 Underlays for walls and the CE-
industries and everyday life. Founded in 1962, the marking. For the application and use the respective
company’s location in Luxembourg manufactures a national provisions apply.
wide range of products among which Tyvek®, a 100%
synthetic material made from high-density spunbonded 2.3 Application
polyethylene fibres. Tyvek® underlays are used in roofs and walls. They
constitute the second water-shedding layer and at the
2.2 Product description/Product definition same time protect the insulation from trapped
DuPont™ Tyvek® is a nonwoven material made of moisture, wind penetration, dust and insects. Insulation
HDPE, which is diffusion open but watertight. It is used installed below Tyvek® is kept dry and performs as
as a roof and wall underlay. designed.
For the placing on the market of the product in the
European Union/European Free Trade Association 2.4 Technical Data
(EU/EFTA) (with the exception of Switzerland) The following chapter comprises technical data for the
Regulation (EU) No. 305/2011 (CPR) applies. The characteristics listed in the Declaration of Performance
product needs a declaration of performance taking into according to the harmonized technical specifications
consideration EN 13859-1:2010 Flexible sheets for EN 13859-1 and EN 13859-2.
waterproofing - Definitions and characteristics of
underlays - Part 1: Underlays for discontinuous roofing Technical Data
2 Environmental Product Declaration DuPont de Nemours (Luxembourg) s.à r.l. – Tyvek® Monolayer 60 (1060B, 1560B,
2460B)
Name Value Unit knife or scissors to cut the sheet as well as a stapler to
50m fix it to the construction. Refer to Tyvek® installation
Length acc. to EN 1848-2 m
standard guidelines attached to every roll for more information.
1.5m
Width acc. to EN 1848-2 m
standard 2.10 Packaging
Grammage acc. to EN 1849-2 0.058 kg/m2 Tyvek® is wound onto carton cores. Each roll comes
Resistance to water penetration with a paper insert sheet. Rolls are individually
W1 -
acc. to EN 1928 (class) wrapped in foil (LDPE: low-density PE) and stacked on
Water vapor diffusion equivalent wooden pallets which are also wrapped in LDPE
air layer thickness acc. to EN ISO 0.015 m stretch film. Vertical sides of the pallets are protected
12572 with a carton profile.
Maximum tensile force acc. to EN All packaging materials can be reused (e.g. pallets),
12311-1 165/135 N/50mm recycled or valorised through energy recovery.
Elongation acc. to EN 12311-1 9/14.5 %
Resistance to water penetration
2.11 Condition of use
after ageing acc. to EN 1297, EN W1 -
Materials are not expected to change or react during
1928 (class)
the period of use. Tyvek® is intended to be installed on
Tear Resistance (nail) acc. to EN
60/60 N the cold side of the insulation and is designed to
12310-1
withstand substantial temperature changes during
service life.
Performance data of the product in accordance with
2.12 Environment and health during use
the declaration of performance with respect to its
Tyvek® membranes are usually concealed below roof
essential characteristics according to EN 13859-
decking or facade cladding. They do not require
1:2010 Flexible sheets for waterproofing - Definitions
maintenance and will not produce emissions. There
and characteristics of underlays - Part 1: Underlays for
are no environmental or health concerns to be
discontinuous roofing and EN 13859-2:2010 Flexible
expected from the use of the material.
sheets for waterproofing - Definitions and
characteristics of underlays - Part 2 Underlays for
walls.
2.13 Reference service life
The documentation of the RSL is not required for this
2.5 Delivery status
EPD since not the entire life cycle is declared (without
The single selling unit is a roll of up to 3 m width and a
modules B1-B7). Nevertheless, the product is
length of up to 100 m. Usually several rolls are
assumed to have a reference service life of 30 years,
strapped and piled on a wooden pallet.
corresponding to the average roof lifetime (BNB
The order unit is square meter [m²].
Nutzungsdauerliste). But this assumption could not be
verified because the Tyvek® envelopes have only
2.6 Base materials/Ancillary materials
been sold for about 25 years.
Tyvek® single layer membranes are made of
- high density polyethylene (HDPE) >99 %
- hindered amine light stabilizers (HALS, added for UV
2.14 Extraordinary effects
stabilization) <1 %.
Fire
2.7 Manufacture
Tyvek® underlays are produced on semi-continuously
operating production facilities in different countries.
Fire protection
Process steps include:
Name Value
Building material class acc. to EN E (on mineral wool
1. Spinning of thin HDPE filaments.
13501-1 and wood)
2. Bonding of filament sheet.
3. Printing, slitting and packaging of the finished roll
Water
goods.
Tyvek® membranes are inherently waterproof. No part
of the product will dissolve in water nor will the product
2.8 Environment and health during
release any toxic substances to water.
manufacturing
The Tyvek® manufacturing facilities employed in the
Mechanical destruction
production of Tyvek® in Luxembourg are ISO
No possible impacts on the environment following
14001 certified. All facilities comply with local
unforeseeable mechanical destruction are known.
regulations and DuPont internal standards. Particular
care is taken to ensure the safety of anyone involved in
2.15 Re-use phase
the Tyvek® supply chain in line with the DuPont safety
The material is not intended to be re-used or recycled.
culture: all injuries can be prevented (goal is ZERO).
Energy recovery is possible.
2.9 Product processing/Installation
2.16 Disposal
Tyvek® membranes for walls and roofs can be either
Disposal of the material should be made according to
installed on the construction site or in manufacturing
national legislation. Incineration is the preferred way of
facilities in case of pre-fabricated buildings. In both
disposal. European Waste Codes (Commission
instances, the material is usually installed by manually
decision 2014/955/EU) for waste plastics (except
unwinding the sheet from the roll and placing it onto
packaging) is 02 01 04 and for mixed construction and
the designated surface. Tools required are usually a
demolition wastes it is 17 09 04. Both may apply.
3 Environmental Product Declaration DuPont de Nemours (Luxembourg) s.à r.l. – Tyvek® Monolayer 60 (1060B, 1560B,
2460B)
Data Sheets (SDS) or Article Information Sheets (AIS)
2.17 Further information of the products can be found at www.dupont.com.
Additional information about product properties and
use can be found at www.building.dupont.com.Safety
3. LCA: Calculation rules
3.1 Declared Unit 3.5 Background data
This declaration applies to 1 m2 of DuPont™ Tyvek® All background data for the LCA model were taken
1060B, 1560B and 2460B membranes, with a declared from the database of GaBi 10.5.0.78.
unit weight of 58 g/m2.
The product 1060B uses a different bonder for 3.6 Data quality
processing, while the products 1560B and 2460B only To simulate the product stage, data recorded by
differ from the printed pattern. DuPont Luxembourg s.à r.l. and the converting plant in
Germany from the production year 2019 were used.
Declared Unit Eurostat data for the years 2018-2019 were used to
Name Value Unit model the modules A4 (freight transport modal split)
Declared unit 1 m2 and A5 (packaging disposal routes).
Grammage 0.058 kg/m2 Regarding background processes, the Luxembourg
and German electricity grid mix were applied to the
production plants in these countries (A1-A3). Other
background data were specific to Germany or the
3.2 System boundary European average, and were not older than 10 years.
Type of EPD: Cradle-to-gate (with options) The representativeness can be classified as very good
The system boundaries of the EPD follow the modular for all the foreground data, and most of the background
construction system as described by EN 15804. The data.
LCA takes into account the following modules:
 A1-A3: Manufacturing of pre-products, 3.7 Period under review
The period of study encompasses the year 2019.
packaging, ancillary materials, transport to the
factory, production including energy supply
3.8 Allocation
and waste handling
Mass allocation was applied for production. At the
 A4: Transport to the construction site DuPont site in Luxembourg, Tyvek® waste materials
 A5: Installation into the building (disposal of are recycled internally or sold and transformed
packaging) externally. The further use of the valorized HDPE
granulates was cut-off from the system boundaries, as
 C4: Waste disposal (incineration)
for the packaging materials sent for recycling. The
 D: Potential for reuse, recovery and/or
Tyvek® final waste material sent to incineration is
recycling (benefits for incineration and modelled through the combustion process of the
recovery of packaging materials from module specific material and the avoided conventional energy
A5 and envelopes incineration from module production is considered in module D. The potential
C4). benefit in module D will be possible only if the Tyvek®
will be separate and incinerated.
3.9 Comparability
3.3 Estimates and assumptions
Basically, a comparison or an evaluation of EPD data
The colour paste used in the finishing process was
is only possible if all the data sets to be compared
valued with a general composition of water-based
were created according to EN 15804 and the building
colour paste (conservative approach).
context, respectively the product-specific
characteristics of performance, are taken into account.
3.4 Cut-off criteria
All data were taken into consideration (recipe
GaBi 10.5.0.78 was used to model background data.
constituents, process water, electricity used). In case
of missing data, a cut-off criteria of 1 % of the total
input mass was applied for unit processes and 5 % for
the entire modules (as recommended by EN 15804,
section 6.3.5) and therefore some inputs were
excluded: tape and spiking agent for monolayer
production (sum < 0.04 % of total input mass for
monolayer production), paper ink, hotmelt, paper, tape
and detergent for finishing process (sum < 0. 2 % of
total input mass for finishing process). Transports were
considered for all inputs and outputs. Manufacturing of
the production machines and systems and associated
infrastructure were not taken into account in the life
cycle assessment (LCA). Regarding possible off-cuts
during installation, the amount is lower than 5 % and
therefore also neglected.
4 Environmental Product Declaration DuPont de Nemours (Luxembourg) s.à r.l. – Tyvek® Monolayer 60 (1060B, 1560B,
2460B)
4. LCA: Scenarios and additional technical information
Characteristic product properties
Information on biogenic Carbon
The product does not contain biogenic carbon.
Information on describing the biogenic Carbon
Content at factory gate
Name Value Unit
Biogenic Carbon Content in
0 kg C
product
Biogenic Carbon Content in
0.0037 kg C
accompanying packaging
The following technical information serves as a basis
for the declared modules or can be used for the
development of specific scenarios in the context of a
building assessment.
Transport from the gate to the construction site
(A4)
Name Value Unit
Transport distance (weighted
3064 km
average)
Transport (train) 1.48E-02 tkm
Transport (road) 6.43E-02 tkm
Transport (water) 1.19E-01 tkm
Installation of the product into the building (A5)
Name Value Unit
Wood waste to landfill 2.97E-4 kg
Wood waste to incineration 1.78E-04 kg
Cardboard waste to landfill 2.96E-04 kg
Cardboard waste to incineration 2.26E-04 kg
Plastic waste to landfill 2.66E-05 kg
Plastic waste to incineration 3.63E-05 kg
End-of-life stage (C1-C4)
Name Value Unit
Collected separately Tyvek® waste 0.058 kg
Energy recovery 100 %
R1 value < 0.6
5 Environmental Product Declaration DuPont de Nemours (Luxembourg) s.à r.l. – Tyvek® Monolayer 60 (1060B, 1560B,
2460B)
5. LCA: Results
The results displayed below apply to 1 m2 of DuPont™ Tyvek® 1060B, 1560B and 2460B membranes, with a
declared unit weight of 58 g/m2.
Disclaimers:
EP-freshwater: This indicator has been calculated as “kg P eq” as required in the characterization model
(EUTREND model, Struijs et al., 2009b, as implemented in ReCiPe;
http://eplca.jrc.ec.europa.eu/LCDN/developerEF.xhtml).
Potential Human exposure efficiency relative to U235: This impact category deals mainly with the eventual impact
of low dose ionizing radiation on human health of the nuclear fuel cycle. It does not consider effects due to
possible nuclear accidents, occupational exposure nor due to radioactive waste disposal in underground facilities.
Potential ionizing radiation from the soil, from radon and from some construction materials is also not measured
by this indicator.
Abiotic depletion potential for non-fossil resources; Abiotic depletion potential for fossil resources; Water (user)
deprivation potential, deprivation-weighted water consumption: The results of these environmental impact
indicators shall be used with care as the uncertainties on these results are high or as there is limited experience
with the indicator.
DESCRIPTION OF THE SYSTEM BOUNDARY (X = INCLUDED IN LCA; ND = MODULE OR INDICATOR NOT
DECLARED; MNR = MODULE NOT RELEVANT)
BENEFITS AND
CONSTRUCTI LOADS
PRODUCT STAGE ON PROCESS USE STAGE END OF LIFE STAGE BEYOND THE
STAGE SYSTEM
BOUNDARIES
6 Environmental Product Declaration DuPont de Nemours (Luxembourg) s.à r.l. – Tyvek® Monolayer 60 (1060B, 1560B,
2460B)
lairetam
waR
ylppus tropsnarT
gnirutcafunaM
eht
morf
tropsnarT
etis
eht
ot
etag
ylbmessA esU
ecnanetniaM
riapeR
tnemecalpeR tnemhsibrufeR
ygrene
lanoitarepO esu
retaw
lanoitarepO esu
noitcurtsnoc-eD
noitilomed tropsnarT
gnissecorp
etsaW
lasopsiD -esueR -yrevoceR -gnilcyceR laitnetop
A1 A2 A3 A4 A5 B1 B2 B3 B4 B5 B6 B7 C1 C2 C3 C4 D
X X X X X ND ND MNR MNR MNR ND ND ND ND ND X X
RESULTS OF THE LCA - ENVIRONMENTAL IMPACT according to EN 15804+A2: 1 m2 DuPont™ Tyvek®
Monolayer 60 (1060B, 1560B and 2460B)
Core Indicator Unit A1-A3 A4 A5 C4 D
Global warming potential - total [kg CO2-Eq.] 2.81E-1 6.04E-3 1.85E-3 1.82E-1 -9.61E-2
Global warming potential - fossil fuels [kg CO2-Eq.] 2.81E-1 5.92E-3 1.50E-4 1.82E-1 -9.56E-2
Global warming potential - biogenic [kg CO2-Eq.] 1.78E-4 8.27E-5 1.70E-3 6.04E-6 -4.49E-4
GWP from land use and land use change [kg CO2-Eq.] 2.10E-4 4.02E-5 4.91E-8 9.74E-7 -6.03E-5
Depletion potential of the stratospheric ozone layer [kg CFC11-Eq.] 4.18E-12 4.77E-18 2.39E-19 1.36E-17 -9.89E-16
Acidification potential, accumulated exceedance [mol H+-Eq.] 1.08E-3 6.60E-5 3.89E-7 1.81E-5 -1.18E-4
Eutrophication, fraction of nutrients reaching freshwater
end compartment
[kg PO4-Eq.] 4.41E-7 1.51E-8 3.68E-9 1.82E-9 -1.14E-7
Eutrophication, fraction of nutrients reaching marine end
[kg N-Eq.] 1.72E-4 2.40E-5 1.70E-7 3.80E-6 -3.45E-5
compartment
Eutrophication, accumulated exceedance [mol N-Eq.] 1.86E-3 2.64E-4 1.58E-6 8.49E-5 -3.70E-4
Formation potential of tropospheric ozone photochemical
[kg NMVOC-Eq.] 6.10E-4 5.41E-5 6.85E-7 1.13E-5 -9.72E-5
oxidants
Abiotic depletion potential for non-fossil resources [kg Sb-Eq.] 4.29E-8 4.51E-10 5.04E-12 2.06E-10 -1.48E-8
Abiotic depletion potential for fossil resources [MJ] 6.99E+0 8.00E-2 8.54E-4 2.22E-2 -1.65E+0
Water (user) deprivation potential, deprivation-weighted [m³ world-Eq
2.60E-2 7.10E-5 8.61E-5 1.67E-2 -6.55E-3
water consumption (WDP) deprived]
RESULTS OF THE LCA - INDICATORS TO DESCRIBE RESOURCE USE according to EN 15804+A2: 1 m2
DuPont™ Tyvek® Monolayer 60 (1060B, 1560B and 2460B)
Indicator Unit A1-A3 A4 A5 C4 D
Renewable primary energy as energy carrier [MJ] 6.28E-1 5.05E-3 8.75E-5 4.39E-3 -3.39E-1
Renewable primary energy resources as material utilization [MJ] 3.23E-4 -9.39E-15 -1.22E-16 1.82E-14 -6.85E-13
Total use of renewable primary energy resources [MJ] 6.28E-1 5.05E-3 8.75E-5 4.39E-3 -3.39E-1
Non-renewable primary energy as energy carrier [MJ] 6.99E+0 8.01E-2 8.54E-4 2.22E-2 -1.65E+0
Non-renewable primary energy as material utilization [MJ] 1.55E-4 2.57E-6 1.67E-8 7.84E-7 -5.37E-5
Total use of non-renewable primary energy resources [MJ] 6.99E+0 8.01E-2 8.54E-4 2.22E-2 -1.65E+0
Use of secondary material [kg] 3.58E-3 0.00E+0 0.00E+0 0.00E+0 0.00E+0
Use of renewable secondary fuels [MJ] 5.65E-8 0.00E+0 0.00E+0 0.00E+0 0.00E+0
Use of non-renewable secondary fuels [MJ] 6.23E-7 0.00E+0 0.00E+0 0.00E+0 0.00E+0
Use of net fresh water [m³] 3.96E-3 5.56E-6 2.05E-6 3.92E-4 -3.31E-4
RESULTS OF THE LCA – WASTE CATEGORIES AND OUTPUT FLOWS according to EN 15804+A2:
1 m2 DuPont™ Tyvek® Monolayer 60 (1060B, 1560B and 2460B)
Indicator Unit A1-A3 A4 A5 C4 D
Hazardous waste disposed [kg] 1.64E-9 4.16E-12 1.54E-13 3.96E-12 -3.67E-10
Non-hazardous waste disposed [kg] 2.86E-3 1.30E-5 4.46E-4 7.20E-4 -7.26E-4
Radioactive waste disposed [kg] 1.21E-4 5.40E-7 1.79E-8 1.26E-6 -1.09E-4
Components for re-use [kg] 0.00 0.00 0.00 0.00 0.00
Materials for recycling [kg] 0.00 0.00 0.00 0.00 0.00
Materials for energy recovery [kg] 0.00 0.00 0.00 0.00 0.00
Exported electrical energy [MJ] 0.00E+0 0.00E+0 1.46E-3 3.88E-1 0.00E+0
Exported thermal energy [MJ] 0.00E+0 0.00E+0 2.08E-3 6.98E-1 0.00E+0
RESULTS OF THE LCA – additional impact categories according to EN 15804+A2-optional:
1 m2 DuPont™ Tyvek® Monolayer 60 (1060B, 1560B and 2460B)
Indicator Unit A1-A3 A4 A5 C4 D
Potential incidence of disease due to PM emissions [Disease
ND ND ND ND ND
Incidence]
Potential Human exposure efficiency relative to U235 [kBq U235-
ND ND ND ND ND
Eq.]
Potential comparative toxic unit for ecosystems [CTUe] ND ND ND ND ND
Potential comparative toxic unit for humans - cancerogenic [CTUh] ND ND ND ND ND
Potential comparative toxic unit for humans - not cancerogenic [CTUh] ND ND ND ND ND
Potential soil quality index [-] ND ND ND ND ND
7 Environmental Product Declaration DuPont de Nemours (Luxembourg) s.à r.l. – Tyvek® Monolayer 60 (1060B, 1560B,
2460B)
6. LCA: Interpretation
The following chart shows the relative contributions of
the different modules to the various LCA categories in
a dominance analysis.
For most of the impact categories, more than 70 % of
the impacts are dominated by the Tyvek® production ADPE: Abiotic depletion potential for non-fossil
(A1-A3) and in particular by the supply of HDPE resources
granulates, steam and electricity. ADPF: Abiotic depletion potential for fossil resources
The production phase represents 59 % of GWP, which AP: Acidification potential, accumulated exceedance
is also highly influenced by the final disposal (39 % of FEP: Eutrophication, fraction of nutrients reaching
the generated impact). This is due to the emissions of freshwater end compartment
carbon dioxide from the incineration plant. Fin.: Finishing process
The avoided energy production thanks to waste GWP: Global Warming Potential
incineration leads to significant benefits, which are HDPE: High-Density Polyethylene
mostly around 20 % of the impact results. LCA: Life Cycle Assessment
Waste incineration during the finishing step, including MEP: Eutrophication, fraction of nutrients reaching
Tyvek® and packaging materials, is completely marine end compartment
dominating the ODP score due to halogens emissions Mono: Monolayer production
to air in the module „EU-28: Waste incineration of Nat. gas: Natural gas
plastics (PE, PP, PS, PB)“. The transport of Tyvek® ODP: Depletion potential of the stratospheric ozone
products to the customers contributes to 12 % of MEP layer
and TEP due to the emissions of nitrogen monoxide POCP: Formation potential of tropospheric ozone
during lorry and sea transport (module A4). As photochemical oxidants
expected, the use of water, in particular cold water for TEP: Eutrophication, accumulated exceedance
monolayer production, dominates the WDP score. WDP: Water (user) deprivation potential, deprivation-
weighted water consumption
Glossary:
7. Requisite evidence
No requisite evidence is required for DuPont™ Tyvek®
1060B, 1560B and 2460B monolayer membranes.
8 Environmental Product Declaration DuPont de Nemours (Luxembourg) s.à r.l. – Tyvek® Monolayer 60 (1060B, 1560B,
2460B)
8. References
EN 12310-1
EN 12310-1:1999, Flexible sheets for waterproofing - ISO 14025
Part 1: Bitumen sheets for roof waterproofing; DIN EN ISO 14025:2011-10, Environmental labels and
determination of resistance to tearing (nail shank) declarations — Type III environmental declarations —
Principles and procedures.
EN 12311-1
EN 12311-1:1999, Flexible sheets for waterproofing - PCR, Part A
Part 1: Bitumen sheets for roof waterproofing; PCR 2021, Part A - PCR Guidance-Calculation Rules
Determination of tensile properties for the Life Cycle Assessment and Requirements on
the Project Report according to EN 15804+A2:2019
EN 1297 (version 1.1.1, 2021)
EN 1297:2004, Flexible sheets for waterproofing -
Bitumen, plastic and rubber sheets for roof PCR, Part B
waterproofing - Method of artificial ageing by long term PCR 2017, Part B - PCR Guidance-Texts for Building-
exposure to the combination of UV radiation, elevated Related Products and Services: Requirements on the
temperature and water EPD for False ceiling and underlay sheeting (version
1.6, 2017)
EN 13501-1
EN 13501-1:2007+A1:2010, Fire classification of IBU 2016
construction products and building elements - Part 1: Institut Bauen und Umwelt e.V.: General Programme
Classification using data from reaction to fire tests Instructions for the Preparation of EPDs at the Institut
Bauen und Umwelt e.V. Version 1., Berlin: Institut
EN 13859-1 Bauen und Umwelt e.V., 2016. www.ibu-epd.com
EN 13859-1:2010, Flexible sheets for waterproofing -
Definitions and characteristics of underlays - Part 1: BNB Nutzungsdauerliste
Underlays for discontinuous roofing BNB Nutzungsdauerliste: 2017. Nutzungsdaueren von
Bauteilen published by Informationsportal Nachhaltiges
EN 13859-2 Bauen des Bundesministeriums des Inneren für Bau
EN 13859-2:2010, Flexible sheets for waterproofing - und Heimat.
Definitions and characteristics of underlays - Part 2:
Underlays for walls European Waste Code
European Waste Code:2000. European List of
EN 15804 Waste European Waste Codes: (Commission decision
EN 15804:2019+A2, Sustainability of construction 2014/955/EU)
works — Environmental Product Declarations — Core
rules for the product category of construction products. Eurostat
Eurostat:2021, Data browser, Packaging waste by
EN 1848-2 waste management operations; Recycling rate of
EN 1848-2:2001, Flexible sheets for waterproofing - packaging waste by type of packaging
Determination of length, width, straightness and
flatness - Part 2: Plastic and rubber sheets for roof GaBi 10.5.0.78
waterproofing GaBi 10.5.0.78:2021. Life Cycle Engineering software
and database. Sphera Solutions GmbH, 2021.
EN 1849-2
EN 1849-2:2019, Flexible sheets for waterproofing - Regulation (EU) No. 305/2011
Determination of thickness and mass per unit area - Regulation (EU) No. 305/2011 of the European
Part 2: Plastic and rubber sheets Parliament and of the Council of 9 March 2011 laying
down harmonised conditions for the marketing of
EN 1928 construction products and repealing Council Directive
EN 1928:2000, Flexible sheets for waterproofing - 89/106/EEC
Bitumen, plastic and rubber sheets for roof
waterproofing - Determination of watertightness DuPont™, the DuPont Oval Logo, and all
trademarks and service marks denoted with ™, SM
EN ISO 12572 or ® are owned by affiliates of DuPont de Nemours,
EN ISO 12572:2017, Hygrothermal performance of Inc. unless otherwise noted.
building materials and products -- Determination of
water vapour transmission properties
EN ISO 14001
EN ISO 14001:2015, Environmental management
systems - Requirements with guidance for use
(ISO 14001:2015)
9 Environmental Product Declaration DuPont de Nemours (Luxembourg) s.à r.l. – Tyvek® Monolayer 60 (1060B, 1560B,
2460B)
Publisher
Institut Bauen und Umwelt e.V. Tel +49 (0)30 3087748- 0
Panoramastr. 1 Fax +49 (0)30 3087748- 29
10178 Berlin Mail info@ibu-epd.com
Germany Web www.ibu-epd.com
Programme holder
Institut Bauen und Umwelt e.V. Tel +49 (0)30 - 3087748- 0
Panoramastr 1 Fax +49 (0)30 – 3087748 - 29
10178 Berlin Mail info@ibu-epd.com
Germany Web www.ibu-epd.com
Author of the Life Cycle
Assessment Tel 00352-275888-1
Luxembourg Institute of Science Fax 00352-275888-555
and Technology (LIST) Mail info@list.lu
Avenue des Hauts-Fourneaux 5 Web www.list.lu
4362 Esch/Alzette
Luxembourg
Owner of the Declaration
DuPont de Nemours (Luxembourg) Tel +352 3666 5210
s.à r.l. Fax +352 3666 0000
Rue Général Patton 1 Mail tyvek.info@dupont.com
2984 Contern Web www.dupont.com
Luxembourg
