ENVIRONMENTAL PRODUCT DECLARATION
as per ISO 14025 and EN 15804+A2
Owner of the Declaration dormakaba International Holding GmbH
Publisher Institut Bauen und Umwelt e.V. (IBU)
Programme holder Institut Bauen und Umwelt e.V. (IBU)
Declaration number EPD-DOR-20210232-CBC1-EN
Issue date 01.10.2021
Valid to 30.09.2026
Reversible Single Cylinder - ace JP, ace APAC
dormakaba
www.ibu-epd.com | https://epd-online.com
General Information
dormakaba Reversible Single Cylinder - ace JP, ace APAC
Programme holder Owner of the declaration
IBU – Institut Bauen und Umwelt e.V. dormakaba International Holding GmbH
Hegelplatz 1 DORMA Platz 1
10117 Berlin 58256 Ennepetal
Germany Germany
Declaration number Declared product / declared unit
EPD-DOR-20210232-CBC1-EN 1 piece of the product: ace JP mechanical key system, consisting of the
following items:
- one (1) ace JP single cylinder
- three (3) ace reversible key
- one (1) user manual
- packaging
This declaration is based on the product category rules: Scope:
Building Hardware products, 01.08.2021 This declaration is a specific product declaration for the ace JP single
(PCR checked and approved by the SVR) cylinder including three keys. This Environmental Product Declaration is
also representative for the system ace APAC. The underlying life cycle
assessment is based on the entire life cycle of this specific mechanical key
Issue date system. Data represents the year 2021. The products are manufactured at
the dormakaba production facilities Wah Yuet in Hong Kong (China).
01.10.2021
The owner of the declaration shall be liable for the underlying information
and evidence; the IBU shall not be liable with respect to manufacturer
information, life cycle assessment data and evidences.
Valid to
30.09.2026 The EPD was created according to the specifications of EN 15804+A2. In
the following, the standard will be simplified as EN 15804.
Verification
The standard EN 15804 serves as the core PCR
Independent verification of the declaration and data according to ISO
14025:2011
internally X externally
Dipl.-Ing. Hans Peters
(Chairman of Institut Bauen und Umwelt e.V.)
Florian Pronold Dr.-Ing. Wolfram Trinius,
(Managing Director Institut Bauen und Umwelt e.V.) (Independent verifier)
1 Environmental Product Declaration - dormakaba - Reversible Single Cylinder - ace JP, ace APAC
Product
• Three rows of pins with up to 16 simultaneously usable
Product description/Product definition
pin positions.
Information about the enterprise
• Pins that make contact with the key are manufactured
dormakaba stands for a broad offering of products, solutions
from wear-resistant hardened steel.
and services for smart and secure access to buildings and
Delivery status:
rooms from a single source.
The declared ace JP, mechanical master key system including
cylinder, key, packaging and service instruction will be supplied
Product description/ Product definition
with a weight of 0,279 kg.
ace JP is patented, reversible master key system representing
the premium segment. The patent offers legal protection Base materials/Ancillary materials
against commercial imitation. Duplicate keys are only made by
For the main product components, the ace JP single cylinder
dormakaba itself or by authorized partners and requires
and three reversible keys the composition of the product is the
identification by means of a security card.
following. Same product composition applies for ace APAC:
While ace JP is an in-house system that is exclusively
manufactured in our factories, ace APAC is a partner system
that can also be assembled by authorized dealers.
For placing the mechanical key systems on the market in the
European Union/European Free Trade Association (EU/EFTA,
with the exception of Switzerland) the following legal provisions
apply:
All systems are classified according to the European locking
cylinder standards EN1303 and DIN18252.
dormakaba mechanical cylinders fulfill the material The cylinders and keys contain partial articles which contain
requirements given within the Directive RoHS 2011/65/EU. In substances listed in the Candidate List of REACH Regulation
addition, cylinders are fire protection tested according to EN 1907/2006/EC (date:
1634-1 and EN 1634-2. 19.01.2021) exceeding 0.1 percentage by mass: yes
Application
• Lead (Pb): 7439-92-1 (CAS-No.) is included in some of
The dormakaba reversible cylinder ace JP and ace APAC can
the alloys used. The concentration of lead in each
be used in both residential as well as in the commercial
individual alloy does not exceed 4.0% (by mass).
segment in small and simple as well as in large and complex
applications, thanks to its versatility. Nearly limitless application
The candidate list can be found on the /ECHA/ website
options are possible.
address: https://echa.europa.eu/de/home
Technical Data
Reference service life
ace JP is a high-performance locking system, which fulfils even
The life cycle (security and function) of a lock cylinder is about
the most challenging requirements. The system offers
10-15 years, depending on the application and frequency of
exceptional security thanks to:
use. The cylinders are tested to 100,000 locking cycles
minimum (EN1303). This corresponds to approximately 18
locking cycles per day for 15 years.
LCA: Calculation rules
— A1, raw material extraction, processing and mechanical
Declared Unit treatments, processing of secondary material input (e.g.
The declared unit is 1 piece of the product: ace JP recycling processes), — A2, transport to the manufacturer, —
Declared unit A3, manufacturing and assembly including provision of all
materials, products and energy, as well as waste processing up
Name Value Unit
to the end-of waste state.
Declared unit 1 piece/product
Conversion factor to 1 kg 3.58 - Construction stage - Modules A4-A5
conversion factor - - The construction process stage includes:
Mass of declared product including — A4, transport to the building site;
packaging 0.279 kg — A5, installation into the building;
including provision of all materials, products and energy, as well
as waste processing up to the end-ofwaste state or disposal of
System boundary
final residues during the construction process stage.
The type of EPD is according to EN 15804:
"cradle to gate with options, modules C1–C4, and module D".
End-of-life stage– Modules C1-C4 and D
The following modules are declared: A1-A3, C1-C4, D and
The end-of-life stage includes:
additional modules: A4 + A5
— C1, de-construction, demolition:
— C2, transport to waste processing;
Production - Module A1-A3
— C3, waste processing for reuse, recovery and/or recycling;
The product stage includes:
— C4, disposal; including provision and all transport, provision
2 Environmental Product Declaration - dormakaba - Reversible Single Cylinder - ace JP, ace APAC
of all materials, products and related energy and water use. lifespan: China
Module D (Benefits and loads beyond the system boundary)
Comparability
includes:
— D, recycling potentials, expressed as net impacts and Basically, a comparison or an evaluation of EPD data is only
benefits. possible if all the data sets to be compared were created
according to EN 15804 and the building context, respectively
Geographic Representativeness the product-specific characteristics of performance, are taken
Land or region, in which the declared product system is into account. Background database: GaBi, SP40.
manufactured, used or handled at the end of the product´s
LCA: Scenarios and additional technical information
Installation into the building (A5)
Characteristic product properties of biogenic carbon
Name Value Unit
Information on describing the biogenic Carbon Content at
Waste packaging (paper) 0,02057 kg
factory gate
Waste packaging (plastic) 0,00494 kg
Name ValueUnit
Biogenic carbon content in accompanying kg End of life (C1-C4)
0.01
packaging C C1: The product dismantling from the building is done manually
Note: 1 kg of biogenic carbon is equivalent to 44/12 kg of CO . without environmental burden.
2
Name Value Unit
Collected separately waste type 0.254 kg
The following technical scenario information is required for the
Recycling 0.249 kg
declared modules.
Energy recovery 0.00441 kg
Transport to the building site (A4)
The product is disassembled in a recycling process.
Name Value Unit
Material recycling is then assumed for the metals. The plastic
Litres of fuel (per piece) 0.0015l/100km components are assumed to be incinerated with energy
Transport distance (truck) 900 km recovery.
Transport distance (ship) 3822 km
Reuse, recovery and/or recycling potentials (D), relevant
Capacity utilisation (including empty runs)
51 % scenario information
average
Collection rate is 100%.
Numbers reflect the average transport distances per cylinder.
3 Environmental Product Declaration - dormakaba - Reversible Single Cylinder - ace JP, ace APAC
LCA: Results
Disclaimer EP-freshwater: This indicator has been calculated as 'kg P eq' as required in the characterization model (EUTREND model,
Struijs et al., 2009b, as implemented in ReCiPe; http://eplca.jrc.ec.europa.eu/LCDN/developerEF.xhtml).
DESCRIPTION OF THE SYSTEM BOUNDARY (X = INCLUDED IN LCA; MND = MODULE OR INDICATOR NOT DECLARED; MNR
= MODULE NOT RELEVANT)
Benefits and
Construction loads beyond
Product stage Use stage End of life stage
process stage the system
boundaries
la ire ta m w a Ry lp p u s tro p s n a rT g n iru tc a fu n a M e h t m o rf tro p s n a rTe tis e h t o t e ta g y lb m e s s A e s U e c n a n e tn ia M ria p e R tn e m e c a lp e R tn e m h s ib ru fe R y g re n e la n o ita re p Oe s u re ta w la n o ita re p Oe s u n o itc u rts n o c -e Dn o itilo m e d tro p s n a rT g n is s e c o rp e ts a W la s o p s iD -e s u e R-y re v o c e R-g n ilc y c e Rla itn e to p
A1 A2 A3 A4 A5 B1 B2 B3 B4 B5 B6 B7 C1 C2 C3 C4 D
X X X X X MND MND MNR MNR MNR MND MND X X X X X
RESULTS OF THE LCA - ENVIRONMENTAL IMPACT according to EN 15804+A2: 1 piece, Reversible Single Cylinder - ace JP,
ace APAC
Parameter Unit A1-A3 A4 A5 C1 C2 C3 C4 D
GWP-total kg CO 2 eq 1.16E+00 6E-02 4.2E-02 0 1E-03 1.1E-02 0 -6.71E-01
GWP-fossil kg CO 2 eq 1.19E+00 5.7E-02 1.3E-02 0 1E-03 1.1E-02 0 -6.69E-01
GWP-biogenic kg CO 2 eq -3.05E-02 2E-03 2.8E-02 0 4.9E-05 2.61E-07 0 -8.19E-04
GWP-luluc kg CO 2 eq 1.1E-03 1.35E-06 1.19E-06 0 2.52E-08 6.34E-07 0 -6.43E-04
ODP kg CFC11 eq 2.37E-13 6.01E-18 1.16E-17 0 1.12E-19 5.65E-18 0 -3.17E-15
AP mol H+ eq 6.25E-03 1.79E-04 1.04E-05 0 1.06E-06 2E-06 0 -5E-03
EP-freshwater kg P eq 3.27E-06 1.23E-08 2.04E-09 0 2.27E-10 9.02E-10 0 -1.65E-06
EP-marine kg N eq 1.2E-03 4.94E-05 3.45E-06 0 3.38E-07 4.5E-07 0 -4.59E-04
EP-terrestrial mol N eq 1.36E-02 5.45E-04 4.7E-05 0 3.75E-06 9.09E-06 0 -5E-03
kg NMVOC
POCP 4.18E-03 1.4E-04 9.21E-06 0 9.55E-07 1.25E-06 0 -2E-03
eq
ADPE kg Sb eq 7.13E-04 1.7E-09 1.7E-10 0 3.18E-11 7.75E-11 0 -3.09E-04
ADPF MJ 1.7E+01 8.05E-01 1.5E-02 0 1.5E-02 5E-03 0 -8.19E+00
m3 world eq
WDP 3.94E-01 1.12E-04 5E-03 0 2.08E-06 1E-03 0 -1.96E-01
deprived
GWP = Global warming potential; ODP = Depletion potential of the stratospheric ozone layer; AP = Acidification potential of land and water; EP =
Eutrophication potential; POCP = Formation potential of tropospheric ozone photochemical oxidants; ADPE = Abiotic depletion potential for non-fossil
resources; ADPF = Abiotic depletion potential for fossil resources; WDP = Water (user) deprivation potential)
RESULTS OF THE LCA - INDICATORS TO DESCRIBE RESOURCE USE according to EN 15804+A2: 1 piece, Reversible Single
Cylinder - ace JP, ace APAC
Parameter Unit A1-A3 A4 A5 C1 C2 C3 C4 D
PERE MJ 4.78E+00 3E-03 2.5E-01 0 4.74E-05 1E-03 0 -1.68E+00
PERM MJ 2.47E-01 0 -2.47E-01 0 0 0 0 0
PERT MJ 5.03E+00 3E-03 3E-03 0 4.74E-05 1E-03 0 -1.68E+00
PENRE MJ 1.66E+01 8.06E-01 2.27E-01 0 1.5E-02 1.95E-01 0 -8.2E+00
PENRM MJ 4.02E-01 0 -2.12E-01 0 0 -1.9E-01 0 0
PENRT MJ 1.7E+01 8.06E-01 1.5E-02 0 1.5E-02 5E-03 0 -8.2E+00
SM kg 5.4E-02 0 0 0 0 0 0 0
RSF MJ 0 0 0 0 0 0 0 0
NRSF MJ 0 0 0 0 0 0 0 0
FW m3 8.59E-03 4.57E-06 1.16E-04 0 8.5E-08 2.74E-05 0 -5E-03
PERE = Use of renewable primary energy excluding renewable primary energy resources used as raw materials; PERM = Use of renewable primary
energy resources used as raw materials; PERT = Total use of renewable primary energy resources; PENRE = Use of non-renewable primary energy
excluding non-renewable primary energy resources used as raw materials; PENRM = Use of non-renewable primary energy resources used as raw
materials; PENRT = Total use of non-renewable primary energy resources; SM = Use of secondary material; RSF = Use of renewable secondary fuels;
NRSF = Use of non-renewable secondary fuels; FW = Use of net fresh water
RESULTS OF THE LCA – WASTE CATEGORIES AND OUTPUT FLOWS according to EN 15804+A2:
1 piece, Reversible Single Cylinder - ace JP, ace APAC
Parameter Unit A1-A3 A4 A5 C1 C2 C3 C4 D
HWD kg 2.73E-08 7.82E-11 3.58E-11 0 1.46E-12 1.98E-11 0 -2.26E-07
NHWD kg 1.29E-01 8.24E-05 2E-03 0 1.54E-06 1E-03 0 -2.9E-02
RWD kg 1E-03 8.67E-07 7E-07 0 1.62E-08 1.93E-07 0 -3.6E-04
CRU kg 0 0 0 0 0 0 0 0
MFR kg 0 0 0 0 0 2.49E-01 0 0
MER kg 0 0 0 0 0 0 0 0
4 Environmental Product Declaration - dormakaba - Reversible Single Cylinder - ace JP, ace APAC
EEE MJ 3.02E-04 0 6.7E-02 0 0 0 0 0
EET MJ 5.48E-04 0 1.33E-01 0 0 0 0 0
HWD = Hazardous waste disposed; NHWD = Non-hazardous waste disposed; RWD = Radioactive waste disposed; CRU = Components for re-use;
MFR = Materials for recycling; MER = Materials for energy recovery; EEE = Exported electrical energy; EET = Exported thermal energy
RESULTS OF THE LCA – additional impact categories according to EN 15804+A2-optional:
1 piece, Reversible Single Cylinder - ace JP, ace APAC
Parameter Unit A1-A3 A4 A5 C1 C2 C3 C4 D
Disease
PM 5.52E-08 2.47E-09 7.38E-11 0 5.58E-12 2.55E-11 0 -5.1E-08
incidence
IR kBq U235 eq 1.06E-01 1.24E-04 9.44E-05 0 2.31E-06 1.74E-05 0 -4.1E-02
ETP-fw CTUe 1.04E+01 5.71E-01 7E-03 0 1.1E-02 2E-03 0 -4.32E+00
HTP-c CTUh 8.94E-09 1.07E-11 4.2E-13 0 2E-13 1.69E-13 0 1.95E-09
HTP-nc CTUh 8.7E-08 4.61E-10 2.92E-11 0 8.57E-12 1.71E-11 0 2.34E-07
SQP SQP 8.71E+00 2E-03 4E-03 0 3.86E-05 2E-03 0 -1.67E+00
PM = Potential incidence of disease due to PM emissions; IR = Potential Human exposure efficiency relative to U235; ETP-fw = Potential comparative
Toxic Unit for ecosystems; HTP-c = Potential comparative Toxic Unit for humans (cancerogenic); HTP-nc = Potential comparative Toxic Unit for humans
(not cancerogenic); SQP = Potential soil quality index
Disclaimer 1 – for the indicator “Potential Human exposure efficiency relative to U235”. This impact category deals mainly with the
eventual impact of low-dose ionizing radiation on human health of the nuclear fuel cycle. It does not consider effects due to possible
nuclear accidents, occupational exposure or radioactive waste disposal in underground facilities. Potential ionizing radiation from the
soil, radon and from some construction materials is also not measured by this indicator.
Disclaimer 2 – for the indicators “abiotic depletion potential for non-fossil resources”, “abiotic depletion potential for fossil resources”,
“water (user) deprivation potential, deprivation-weighted water consumption”, “potential comparative toxic unit for ecosystems”,
“potential comparative toxic unit for humans – cancerogenic”, “Potential comparative toxic unit for humans - not cancerogenic”,
“potential soil quality index”. The results of this environmental impact indicator shall be used with care as the uncertainties on these
results are high as there is limited experience with the indicator.
References
DIN 18252 equipment.
DIN 18252:
2018, Profile cylinders for door locks – Terminology, European Chemicals Agency (ECHA)
dimensions, requirements, test methods and marking https://echa.europa.eu/de/
DIN EN 1303 Further References
DIN EN 1303:
2015, Building Hardware - Cylinders for locks - Requirements IBU
and test methods Institut Bauen und Umwelt e.V.:
General Instructions for the EPD Programme of Institut Bauen
DIN EN 1634-1 und Umwelt e.V. Version 2.0., Berlin: Institut Bauen und Umwelt
DIN EN 1634-1:2018, Fire resistance and smoke control tests e.V., 2021.
for door and shutter assemblies, openable windows and www.ibu-epd.com
elements of building hardware
GaBi ts software
DIN EN 1634-2 Sphera Solutions GmbH Gabi Software System and Database
DIN EN 1634-2:2009, Fire resistance and smoke control tests for Life Cycle Engineering 1992-2020 Version 10.0.0.71
for door, shutter and openable window assemblies and University of Stuttgart Leinfelden-Echterdingen
elements of building hardware
GaBi ts documentation
DIN EN ISO 14025 GaBi life cycle inventory data documentation (https://www.gabi-
DIN EN ISO 14025:2011, Environmental labels and software.com/support/gabi/gabidatabase- 2020-lci-
declarations - Type III environmental declarations - Principles documentation/).
and procedures.
LCA-tool dormakaba
EN 15804 LCA tool, version 1.0.
EN 15804:2019+A2, Sustainability of construction works - Developed by Sphera Solutions GmbH
Environmental Product Declarations — Core rules for the
product category of construction products. PCR Part A
PCR – Part A: Calculation Rules for the Life Cycle Assessment
REACH Regulation and Requirements on the Project Re-port according to EN
REACH Regulation (EC) No 1907/2006 of the European 15804+A2:2019, Version 1.0, Institut Bauen und Umwelt e.V.,
Parliament and of the Council on the Registration, Evaluation, www.ibu-epd.com.
Authorisation and Restriction of Chemicals.
PCR Part B
RoHS 2011/65/EU PCR – Part B: Requirements on the EPD for Electronic and
RoHS 2011/65/EU, Directive on the restriction of the use of physical Access Control Systems , version 1.2, Institut Bauen
certain hazardous substances in electrical and electronic und Umwelt e.V., www.ibu-epd.com, 2017.
5 Environmental Product Declaration - dormakaba - Reversible Single Cylinder - ace JP, ace APAC
Publisher
Institut Bauen und Umwelt e.V. +49 (0)30 3087748- 0
Hegelplatz 1 info@ibu-epd.com
10117 Berlin www.ibu-epd.com
Germany
Programme holder
Institut Bauen und Umwelt e.V. +49 (0)30 3087748- 0
Hegelplatz 1 info@ibu-epd.com
10117 Berlin www.ibu-epd.com
Germany
Author of the Life Cycle Assessment
Sphera Solutions GmbH +49 711 341817-0
Hauptstraße 111- 113 info@sphera.com
70771 Leinfelden-Echterdingen www.sphera.com
Germany
Owner of the Declaration
dormakaba International Holding GmbH +49 2333 793-0
DORMA Platz 1 info.de@dormakaba.com
58256 Ennepetal www.dormakaba.com
Germany
6 Environmental Product Declaration - dormakaba - Reversible Single Cylinder - ace JP, ace APAC
