ENVIRONMENTAL PRODUCT DECLARATION
as per ISO 14025 and EN 15804+A2
Owner of the Declaration Stiferite
Publisher Institut Bauen und Umwelt e.V. (IBU)
Programme holder Institut Bauen und Umwelt e.V. (IBU)
Declaration number EPD-STF-20220150-CBC2-EN
Issue date 28.07.2022
Valid to 27.07.2027
Stiferite Class SK120
Stiferite
www.ibu-epd.com | https://epd-online.com
General Information
Stiferite Stiferite Class SK120
Programme holder Owner of the declaration
IBU – Institut Bauen und Umwelt e.V. Stiferite
Hegelplatz 1 Viale Navigazione Interna 54
10117 Berlin 35129 Padova
Germany Italy
Declaration number Declared product / declared unit
EPD-STF-20220150-CBC2-EN STIFERITE CLASS SK (CSK120) expanded rigid polyurethane foam,
covered on both sides by saturated fibre glass facers, and produced by
Stiferite. The EPD applies to 1 m2 of 120 mm thick PUR sandwich board,
i.e. 0.12 m3, with an average density between foam and facing of 34.23
kg/m3.
This declaration is based on the product category rules: Scope:
Insulating materials made of foam plastics, 01.08.2021 Stiferite produces STIFERITE Class SK which is a high performance
(PCR checked and approved by the SVR) insulation board manufactured from closed cell expanded rigid
polyurethane foam, covered on both sides by saturated fibre glass
facers.The data have been provided by the only Stiferite factory that is
Issue date located in Padova (Italy) for the year 2020 and sold worldwide.
The owner of the declaration shall be liable for the underlying information
28.07.2022
and evidence; the IBU shall not be liable with respect to manufacturer
information, life cycle assessment data and evidences.
Valid to
The EPD was created according to the specifications of EN 15804+A2. In
27.07.2027 the following, the standard will be simplified as EN 15804.
Verification
The standard EN 15804 serves as the core PCR
Independent verification of the declaration and data according to ISO
14025:2011
internally X externally
Dipl.-Ing. Hans Peters
(Chairman of Institut Bauen und Umwelt e.V.)
Dipl.-Ing. Hans Peters Prof. Dr. Birgit Grahl,
(Managing Director Institut Bauen und Umwelt e.V.) (Independent verifier)
1 Environmental Product Declaration - Stiferite - Stiferite Class SK120
Product
Product according to the CPR based on a
Product description/Product definition hEN/:13165:2012+A2:2016 For the placing on the market of the
STIFERITE'S thermo insulation panels are mainly used in the product in the European Union/European Free Trade
building/construction sector and in industrial insulation. Association (EU/EFTA) (with the exception of Switzerland)
The panels are made of thermo-setting closed cells Regulation (EU) No.305/2011 (CPR) applies. The product
polyurethane foam (PU) supplied with various types of flexible needs a Declaration of Performance taking into consideration
facers on both sides of the panel. The nature/type of facer is a EN 13165:2012+A2:2016. Thermal insulation products for
function of the type of panel and its application. building- factory made rigid polyurethane foam (PU) products -
Expanded rigid polyurethane foam is distinguished by its Specification and the CE-marking. For the application and use
thermal insulation performance, mechanical resistance, the respective national provisions apply.
workability, lightness, and durability.
The performance of STIFERITE'S panels is determined based Base materials/Ancillary materials
on the European norm EN13165:2012+A2:2016 Thermal Core material (about 96.3 % of the weight of the declared
insulation products for buildings - Factory-made rigid unit):
polyurethane foam (PU) products - Specification.
This EPD refers to STIFERITE's Class SK 120 mm thick panel, Closed-cell Polyiso (PIR) rigid foam made from MDI (50-65 %),
made of an insulation component in polyurethane foam using polyols (20-30 %), pentane (4-5 %) and additives (4-7 %).
blowing agent Pentanebased, covered on both sides by
saturated fibre glass facers.The saturated fibre glass facer Facing (about 3.7 % of the weight of the declared unit):
assures perfect adhesiveness to mortar and rendering layers saturated fibre glass consisting of glass fibre (75-85 %) and
used in External Thermal Insulation Composite Systems urea-formaldehyde (25-15 %).
(ETICS). The PU board for insulation:
The panel is produced in standard dimensions of 600 x 1200
• This product/article/at least one partial article contains
mm and straight finish borders.
substances listed in the candidate list (date: 17.01.2022)
Upon request and for minimum quantities, the panels may be
exceeding 0.1 percentage by mass: no
produced in various dimensions, and the borders may be
rabbeted along the sides. The surface of the panel may be • This product/article/at least one partial article doesn't
evened out with sandpaper in order to allow installation on contain other CMR substances in categories 1A or 1B
uneven surfaces. STIFERITE Class SK panel is produced by a which are not on the candidate list, exceeding 0.1
certified company with systems:ISO 9001, OHSAS 18001, ISO percentage by mass: no
14001 in its entire line of products. • Biocide products were added to this construction
product or it has been treated with biocide products (this
Application
then concerns a treated product as defined by the (EU)
The STIFERITE Class SK panel is recommended in external Ordinance on Biocide Products No.528/2012): no
insulation applications: External walls, ventilated facades, Additional declaration according to quoted law: The product is
correction of thermal bridges and porches. STIFERITE's Class compliant with all requirements indicated in chapter 2.5.7
SK is used in ETICS applications having ETA certification 'Isolanti termici ed acustici' of the n.256 D.L. of the 23th June
issued based on EAD 040083-00-0404. 2022 (CAM EDILIZIA):
• Any blowing agent with Ozone depletion potential >0 is
The STIFERITE Class Class SK is recommended also for
not used in production
insulating: roof(s) and floors under bituminous or synthetic
• Any substances of Very High Concern-SVHC in
waterproof coverings.
concentration of more than 0,1 %w are not used in
Technical Data production (REACH n. 1907/2006). Any specific
In this Life Cycle Assessment, a PU insulation board with the authorizations for use are eserved provided for by the
following properties has been regarded: same Regulation for the substances included in Annex
XIV and specifications restrictions set out in Annex XVII
Constructional data
of the Regulation.
Name Value Unit • Catalysts lead-based are not used in production Flame
Gross density 34.24 kg/m3 retardants used in production (belonging to the
Organophosphorus class) are not banned by any
Declared Average Thermal conductivity λD acc.
0.025 W/mK national or European regulation
to EN 13165
• According to the raw materials declarations of suppliers
Compressive strength at 10% deformation acc. to
>150 kPa the minimum amount of recycled raw materials based
EN 826
on the insulation board (PU foam and facers) weight is 3
Tensile strength perpendicular to the face acc. to >80 kPa %w and the minimum amount of recycled raw materials
EN 1607 based on the PU insulation foam weight is 4 %w in
Water absorption by total immersion acc. to EN Vol.- compliance with REMADE in Italy type 1 certification
<2
12087 % (note: this information is not explicitly considered in the
Water absorption by partial immersion acc. to EN LCA and not included in the EPD tables that only refer
< 0.1 kg/m²
1609 to recycling content in the foreground system).
Water vapour diffusion resistance factor μ acc. to
56 Reference service life
EN 12086
The durability of insulation panels is normally at least as long as
Euroclass reaction to fire acc. to EN 11925 E
the lifetime of the building in which it is used. The experimental
This provides a thermal resistance R = 4.8 m² k/W. data show that the reference life is greater than 50 years.
2 Environmental Product Declaration - Stiferite - Stiferite Class SK120
LCA: Calculation rules
thermal insulation board. The life cycle is split into the following
Declared Unit individual phases:
The declared unit is 1 m² with a thickness of 120 mm, e. g. 0.12 A1 - Raw material formulation
m³. A2 - Raw material transport
Corresponding conversion factors are listed in the table below. A3 - Production of the insulation board and packaging material
Declared unit A4 - Transport to the construction site
C1 - demolition and deconstruction
Name Value Unit
C2 - Transport to end of life
Declared unit 1 m2 C3 - End-of-Life: waste management (thermal recovery)
Gross density 34.24 kg/m3 C4 - End-of-Life: waste management (landfill)
Grammage 4.11 kg/m2 D - Benefits and loads beyond system boundary
Layer thickness 0.12 m Geographic Representativeness
Declared average thermal conductivity λD 0.025 W/mK Land or region, in which the declared product system is
manufactured, used or handled at the end of the product´s
This provides a thermal resistance R = 4.8 m² /W.
lifespan: Italy
Comparability
System boundary
Basically, a comparison or an evaluation of EPD data is only
Type of the EPD: cradle to gate - with options
possible if all the data sets to be compared were created
This life cycle assessment for the production of the
according to EN 15804 and the building context, respectively
polyurethane insulation board considers the life cycle from the
the product-specific characteristics of performance, are taken
supply of raw materials to the manufacturer´s gate (cradle-to-
into account. The background database used is GaBi 2022
gate with options). It also includes the transport to the
database (v. 2022.1)
construction site and the end-of-life stage of the used PU
LCA: Scenarios and additional technical information
Characteristic product properties of biogenic carbon
End of life (C1-C4)
Name Value Unit
Information on describing the biogenic Carbon Content at
Scenario No 1: Material Incineration 100 %
factory gate
Scenario No 1: Landfill 100 %
Name Value Unit
kg C1 – Deconstruction and demolition (0.2 MJ/kg as electrical
Biogenic carbon content in product - C consumption assumed)
Biogenic carbon content in accompanying kg
0.00057 C2 – Panel is transported from the building site to a treatment
packaging C
plant by truck and an average distance of 100 km is
considered.
C3/C4- Disposal scenarios used are divided into 2 sub-
Transport to the building site (A4) scenarios:
1) Incineration 100 % (C3/1)
Name ValueUnit
2) Landfilling 100 % (C4/2)
Truck with a capacity of 17.3 tons 267 km
Ferry with a capacity of 1200-10000 dwt payload D- Benefits and loads beyond system boundary are divided into
13 km
capacity 2 sub-scenarios:
Ship with a capacity of 27500 dwt payload capacity 1) Incineration 100 % (D1)
977 km
tons 2) Landfilling 100 % (D2)
Plane with a capacity of 22 ton 0 km
Reuse, recovery and/or recycling potentials (D), relevant
Type and amount of packaging included in module A3 scenario information
Name Value Unit D: Benefits and loads beyond system boundary are divided into
Cardboard 0.00107 kg 2 sub-scenarios:
EPS stock 0.00604 kg Name Value Unit
EPS stock - glue 0.00031 kg Scenario No 1: Material Incineration 100 %
Paper labels 0.00025 kg Scenario No 2: Landfill 100 %
PE film 0.06914 kg
PP tape 0.00089 kg
PUR stucks 0 kg
SBR labels 0.00001 kg
TOTAL PACKAGING 0.07771 kg
3 Environmental Product Declaration - Stiferite - Stiferite Class SK120
LCA: Results
The tables below show the results of the LCA. Basic information on all declared modules provides chapter 4.
There are two scenarios for the end-of-life (C2, C4 and D) analyzed: Scenario 1 considers 100 % incineration, Scenario 2 considers
100 % landfill disposal.
For SM, RSF, NRSF, CRU indicators only the foreground system is considered.
DESCRIPTION OF THE SYSTEM BOUNDARY (X = INCLUDED IN LCA; ND = MODULE OR INDICATOR NOT DECLARED; MNR =
MODULE NOT RELEVANT)
Benefits and
Construction loads beyond
Product stage Use stage End-of-life stage
process stage the system
boundaries
la ire ta m w a Ry lp p u s tro p s n a rT g n iru tc a fu n a M e h t m o rf tro p s n a rTe tis e h t o t e ta g y lb m e s s A e s U e c n a n e tn ia M ria p e R tn e m e c a lp e R tn e m h s ib ru fe R y g re n e la n o ita re p Oe s u re ta w la n o ita re p Oe s u n o itc u rts n o c -e Dn o itilo m e d tro p s n a rT g n is s e c o rp e ts a W la s o p s iD -e s u e R-y re v o c e R-g n ilc y c e Rla itn e to p
A1 A2 A3 A4 A5 B1 B2 B3 B4 B5 B6 B7 C1 C2 C3 C4 D
X X X X MND MND MND MNR MNR MNR MND MND X X X X X
RESULTS OF THE LCA - ENVIRONMENTAL IMPACT according to EN 15804+A2: 1 m2 CSK120
Parameter Unit A1-A3 A4 C1 C2 C3/1 C3/2 C4/1 C4/2 D/1 D/2
GWP-total kg CO 2 eq 1.18E+01 1.54E-01 9.4E-02 2.49E-02 8.82E+00 0 0 6.37E-02 -4.19E+00 0
GWP-fossil kg CO 2 eq 1.19E+01 1.53E-01 9.4E-02 2.47E-02 8.82E+00 0 0 6.34E-02 -4.19E+00 0
GWP-
biogenic kg CO 2 eq -1.09E-01 3.76E-04 5.55E-05 8E-05 6.22E-04 0 0 1.94E-04 -3.78E-03 0
GWP-luluc kg CO 2 eq 5.63E-03 6.34E-04 6.1E-06 1.66E-04 2.28E-05 0 0 1.13E-04 -2.26E-04 0
ODP kg CFC11 eq 1.6E-11 1.26E-14 9.28E-13 2.42E-15 7.35E-13 0 0 1.46E-13 -3.07E-11 0
AP mol H+ eq 2E-02 2.54E-03 1.38E-04 8.23E-05 5.19E-03 0 0 4.38E-04 -5.17E-03 0
EP-
kg P eq 3.68E-05 3.49E-07 4.22E-08 8.8E-08 2.15E-07 0 0 6.09E-07 -1.46E-06 0
freshwater
EP-marine kg N eq 5.75E-03 7.26E-04 3.77E-05 3.76E-05 2.5E-03 0 0 1.12E-04 -1.51E-03 0
EP-terrestrial mol N eq 5.89E-02 7.98E-03 4.03E-04 4.21E-04 2.88E-02 0 0 1.23E-03 -1.62E-02 0
kg NMVOC
POCP 2.44E-02 1.9E-03 1.07E-04 7.39E-05 6.43E-03 0 0 3.4E-04 -4.29E-03 0
eq
ADPE kg Sb eq 3.43E-06 1.16E-08 1.12E-08 2.48E-09 1.96E-08 0 0 6.41E-09 -4.2E-07 0
ADPF MJ 2.99E+02 1.95E+00 1.99E+00 3.23E-01 2.51E+00 0 0 8.33E-01 -8.32E+01 0
m3 world eq
WDP 2.12E+00 1.16E-03 7.02E-03 2.75E-04 8.81E-01 0 0 6.62E-03 -2.35E-01 0
deprived
GWP = Global warming potential; ODP = Depletion potential of the stratospheric ozone layer; AP = Acidification potential of land and water; EP =
Eutrophication potential; POCP = Formation potential of tropospheric ozone photochemical oxidants; ADPE = Abiotic depletion potential for non-fossil
resources; ADPF = Abiotic depletion potential for fossil resources; WDP = Water (user) deprivation potential)
RESULTS OF THE LCA - INDICATORS TO DESCRIBE RESOURCE USE according to EN 15804+A2: 1 m2 CSK120
Parameter Unit A1-A3 A4 C1 C2 C3/1 C3/2 C4/1 C4/2 D/1 D/2
PERE MJ 1.58E+01 8.83E-02 2.88E-01 2.24E-02 4.34E-01 0 0 1.22E-01 -9.57E+00 0
PERM MJ 2.24E-02 0 0 0 0 0 0 0 0 0
PERT MJ 1.59E+01 8.83E-02 2.88E-01 2.24E-02 4.34E-01 0 0 1.22E-01 -9.57E+00 0
PENRE MJ 1.89E+02 1.96E+00 1.99E+00 3.25E-01 1.1E+02 0 0 1.08E+02 -8.32E+01 0
PENRM MJ 1.11E+02 0 0 0 -1.07E+02 0 0 -1.07E+02 0 0
PENRT MJ 3E+02 1.96E+00 1.99E+00 3.25E-01 2.51E+00 0 0 8.34E-01 -8.32E+01 0
SM kg 3.6E-01 0 0 0 0 0 0 0 0 0
RSF MJ 0 0 0 0 0 0 0 0 0 0
NRSF MJ 0 0 0 0 0 0 0 0 0 0
FW m3 7.25E-02 1.03E-04 4.36E-04 2.59E-05 2.07E-02 0 0 2.02E-04 -1.45E-02 0
PERE = Use of renewable primary energy excluding renewable primary energy resources used as raw materials; PERM = Use of renewable primary
energy resources used as raw materials; PERT = Total use of renewable primary energy resources; PENRE = Use of non-renewable primary energy
excluding non-renewable primary energy resources used as raw materials; PENRM = Use of non-renewable primary energy resources used as raw
materials; PENRT = Total use of non-renewable primary energy resources; SM = Use of secondary material; RSF = Use of renewable secondary fuels;
NRSF = Use of non-renewable secondary fuels; FW = Use of net fresh water
RESULTS OF THE LCA – WASTE CATEGORIES AND OUTPUT FLOWS according to EN 15804+A2:
1 m2 CSK120
Parameter Unit A1-A3 A4 C1 C2 C3/1 C3/2 C4/1 C4/2 D/1 D/2
HWD kg 8.15E-08 9.45E-12 1.42E-10 1.72E-12 3.36E-10 0 0 4.68E-11 -7.88E-09 0
NHWD kg 2.79E-01 2.69E-04 4.24E-04 5.29E-05 1.05E-01 0 0 4.11E+00 -1.85E-02 0
RWD kg 3.39E-03 3.11E-06 3.31E-04 6.02E-07 1.13E-04 0 0 9.35E-06 -1.09E-02 0
CRU kg 0 0 0 0 0 0 0 0 0 0
4 Environmental Product Declaration - Stiferite - Stiferite Class SK120
MFR kg 0 0 0 0 0 0 0 0 0 0
MER kg 0 0 0 0 0 0 0 0 0 0
EEE MJ 0 0 0 0 2.71E+01 0 0 0 0 0
EET MJ 0 0 0 0 1.54E+01 0 0 0 0 0
HWD = Hazardous waste disposed; NHWD = Non-hazardous waste disposed; RWD = Radioactive waste disposed; CRU = Components for re-use;
MFR = Materials for recycling; MER = Materials for energy recovery; EEE = Exported electrical energy; EET = Exported thermal energy
RESULTS OF THE LCA – additional impact categories according to EN 15804+A2-optional:
1 m2 CSK120
Parameter Unit A1-A3 A4 C1 C2 C3/1 C3/2 C4/1 C4/2 D/1 D/2
Disease
PM 1.52E-07 3.87E-08 1.23E-09 4.71E-10 1.5E-08 0 0 5.37E-09 -4.58E-08 0
incidence
IR kBq U235 eq 3.85E-01 4.66E-04 4.85E-02 9.1E-05 1.77E-02 0 0 1.06E-03 -1.6E+00 0
ETP-fw CTUe 1.21E+02 1.37E+00 6.1E-01 2.29E-01 8.6E-01 0 0 1.45E+01 -2.03E+01 0
HTP-c CTUh 9.91E-09 2.72E-11 1.12E-11 4.72E-12 6.21E-11 0 0 6.96E-11 -5.05E-10 0
HTP-nc CTUh 5.95E-07 1.55E-09 5.72E-10 2.89E-10 2.42E-09 0 0 7.66E-09 -2.44E-08 0
SQP SQP 3.09E+01 5.24E-01 1.83E-01 1.37E-01 5.12E-01 0 0 1.68E-01 -6.08E+00 0
PM = Potential incidence of disease due to PM emissions; IR = Potential Human exposure efficiency relative to U235; ETP-fw = Potential comparative
Toxic Unit for ecosystems; HTP-c = Potential comparative Toxic Unit for humans (cancerogenic); HTP-nc = Potential comparative Toxic Unit for humans
(not cancerogenic); SQP = Potential soil quality index
Disclaimer 1 – for the indicator “Potential Human exposure efficiency relative to U235”. This impact category deals mainly with the
eventual impact of low-dose ionizing radiation on human health of the nuclear fuel cycle. It does not consider effects due to possible
nuclear accidents, occupational exposure or radioactive waste disposal in underground facilities. Potential ionizing radiation from the
soil, radon and from some construction materials is also not measured by this indicator.
Disclaimer 2 – for the indicators “abiotic depletion potential for non-fossil resources”, “abiotic depletion potential for fossil resources”,
“water (user) deprivation potential, deprivation-weighted water consumption”, “potential comparative toxic unit for ecosystems”,
“potential comparative toxic unit for humans – cancerogenic”, “Potential comparative toxic unit for humans - not cancerogenic”,
“potential soil quality index”. The results of this environmental impact indicator shall be used with care as the uncertainties on these
results are high as there is limited experience with the indicator.
References
Standards applications. Determination of long term water absorption by
immersion.
CPR
Regulation (EU) No.305/2011 laying down harmonised EN 13165
conditions for the marketing of construction products and EN 13165:2012+A2:2016 Thermal insulation products for
repealing Council Directive 89/106/EEC buildings - Factory made rigid polyurethane foam (PU)
products -Specification
EAD 040083-00-0404
External Thermal Insulation Composite Systems (ETICS) with EN 15804
renderings EN 15804:2012+AC:2021 Sustainability of construction works
— Environmental Product Declarations — Core rules for the
EN 826 product category of construction products.
EN 826:2013 Determination of Compression Behavior of
Thermal Insulation Products ETAG 004
ETAG 004: 2013 External Thermal Insulation Composite
EN 1607 Systems with rendering
EN 1607: 2013 Thermal insulating products for building
applications. Determination of tensile strength perpendicular to ISO 9001
faces ISO 9001:2015 Quality management
EN 1609 ISO 14001
EN 1609: Thermal insulating products for building applications. ISO 14001: 2015 Environmental management systems
Determination of short term water absorption by partial
immersion. ISO 14025
EN ISO 14025:2011 Environmental labels and declarations —
EN 11925 Type III environmental declarations - Principles and procedures.
EN 11925:2010 Reaction to fire tests. Ignitability of products
subjected to direct impingement of flame. Single-flame source OHSAS 18001
test. OHSAS 18001: 2007 Occupational Health and Safety Zone
EN 12086 GaBi 2022
EN 12086: 2013 Thermal insulating products for building GaBi 10 and DB 2022.1: Documentation of GaBi 10: Software-
applications. Determination of water vapour transmission System and Database for Life Cycle Engineering. Copyright,
properties. TM. Stuttgart, Leinfelden-Echterdingen, 1992-2022
http://www.gabi-software.com
EN 12087
EN 12087:2013 Thermal insulating products for building IBU 2021
5 Environmental Product Declaration - Stiferite - Stiferite Class SK120
Institut Bauen und Umwelt e.V.: General Instructions for the
EPD programme of Institut Bauen und Umwelt e.V.,Version 2.0, PANGPP 2017
Berlin: Institut Bauen und Umwelt e.V., 2021 Piano d' Azione Nazionale sul Green Public Procurement
www.ibu-epd.com (PANGPP) – Gazzetta Ufficiale della
Repubblica Italiana, Serie Generale n.23 del 28-01-2017
IBU PCR Part A V2.1 http://www.minambiente.it/sites/default/files/archivio/allegati/GPP/GPP_CAM_Edilizia.pdf
Product Category Rules for Building-Related Products and
Services. Part A: Calculation Rules for the Life Cycle REACH
Assessment and Requirements on the Background Report. REACH Registration, Evaluation, Authorization and Restriction
of Chemical, 2007
IBU PCR Part B
PCR Guidance-Texts for Building-Related Products and REMADE IN ITALY
Services; Part B: Requirements on the EPD for Insulating Certificate No.1245/001 for Stiferite Rev. n. 0 18 November
materials made of foam plastics; Institute Construction and 2021
Environment e.V. (IBU). Version 06.2017
https://epd-online.com STIFERITE LCA tool background report v 2.3 (03-06-2022)
6 Environmental Product Declaration - Stiferite - Stiferite Class SK120
Publisher
Institut Bauen und Umwelt e.V. +49 (0)30 3087748- 0
Hegelplatz 1 info@ibu-epd.com
10117 Berlin www.ibu-epd.com
Germany
Programme holder
Institut Bauen und Umwelt e.V. +49 (0)30 3087748- 0
Hegelplatz 1 info@ibu-epd.com
10117 Berlin www.ibu-epd.com
Germany
Author of the Life Cycle Assessment
Sphera Solutions GmbH +49 711 341817-0
Hauptstraße 111- 113 info@sphera.com
70771 Leinfelden-Echterdingen www.sphera.com
Germany
Owner of the Declaration
Stiferite +39 049 8997911
Viale Navigazione Interna 54 info@stiferite.com
35129 Padova www.stiferite.com
Italy
7 Environmental Product Declaration - Stiferite - Stiferite Class SK120
