ENVIRONMENTAL PRODUCT DECLARATION
as per ISO 14025 and EN 15804+A1
Owner of the Declaration Armstrong World Industries Ltd
Programme holder Institut Bauen und Umwelt e.V. (IBU)
Publisher Institut Bauen und Umwelt e.V. (IBU)
Declaration number EPD-AWI-20200053-ICA1-EN
Issue date 08.01.2020
Valid to 07.01.2025
Ultima+ Planks (19 mm)
Armstrong World Industries Ltd
www.ibu-epd.com | https://epd-online.com
Umwelt Produktdeklaration Name des Herstellers – Name des Produkts
1. General Information
Armstrong World Industries Ltd Ultima+ Planks (19mm)
Programme holder Owner of the declaration
IBU – Institut Bauen und Umwelt e.V. Armstrong World Industries Ltd
Panoramastr. 1 Kingsway South
10178 Berlin Team Valley Trading Estate
Germany Gateshead Tyne & Wear NE11 OSP
Declaration number Declared product / declared unit
EPD-AWI-20200053-ICA1-EN Mineral ceiling tiles (wet felt) 19mm / 1m2
This declaration is based on the product Scope:
category rules: This declaration and its LCA study are based on
Mineral panels, 12.2018 2016 production data for ceiling products manufactured
(PCR checked and approved by the SVR) at the Armstrong Munster plant in Germany.
Issue date The owner of the declaration shall be liable for the
08.01.2020 underlying information and evidence; the IBU shall not
be liable with respect to manufacturer information, life
cycle assessment data and evidences.
Valid to
The EPD was created according to the specifications
07.01.2025
of EN 15804+A1. In the following, the standard will be
simplified as EN 15804.
Verification
The standard EN 15804 serves as the core PCR
Independent verification of the declaration and data
according to ISO 14025:2010
Dipl. Ing. Hans Peters internally x externally
(chairman of Institut Bauen und Umwelt e.V.)
Dr. Alexander Röder Dipl. Natw. ETH Sascha Iqbal
(Managing Director Institut Bauen und Umwelt e.V.)) (Independent verifier appointed by SVR)
2. Product
2.1 Product description/Product definition sound absorption, sound insulation, fire resistance and
very low Volatile Organic Compound (VOC) emissions.
Mineral ceiling tiles and planks are factory produced Typical applications are in offices, schools, healthcare
using the wet felt process. They meet the requirements premises, retail, leisure and transport sectors.
of /DIN 18177/ and are placed on the market in
accordance with /EN 13964/ as well as German 2.3 Technical Data
legislation on hazardous substances. Mineral tiles and
planks consist of mineral wool(s), fillers and binders.
The Ultima+ surface is a smoother finely textured Constructional data (acc. to /EN 13964/)
laminated durable finish and available in a range of
different edge details; Board, Tegular, MicroLook 90,
Vector, and SL2/K2C2. Name Value Unit
Thermal conductivity 0.052 W/(mK)
For the placing on the market of the product in Sound absorption coefficient acc. to
0.65 %
the European Union/European Free Trade Association /EN ISO 354/ and /EN ISO 11654/
(EU/EFTA) (with the exception of Switzerland) Flanking Transmission of Airborne
/Regulation (EU) No. 305/2011 (CPR) / applies. The Sound acc. to /EN ISO 10848-2/ & /EN 40 dB
product needs a Declaration of Performance taking ISO 717-1/
into consideration /EN 13964/ Suspended ceilings - Nominal density 280 kg/m³
Requirements and test methods and the CE marking.
Performance data of the product in accordance with
2.2 Application the declaration of performance with respect to its
essential characteristics according to /EN 13964/ (not
Wet felt mineral suspended ceiling products are used part of CE-marking).
as aesthetic internal ceiling linings and offer
concealment of building services as well as providing
2 Environmental Product Declaration Armstrong World Industries Ltd – Ultima+ planks (19mm)
 Dust and formaldehyde air concentrations in
2.4 Delivery status critical working areas are below the upper
value of occupational exposure
The EPD refers to 19mm thick planks that can have
limits.Exempted from measuring crystalline
varying length and width dimensions.
silica in the air by the competent authorities,
2.5 Base materials/Ancillary materials as historical values measured were lower
than 1/10 of the limit.
Name Value Unit
Binding Agent - mainly starch 0 - 10 %
Armstrong World Industries is /ISO 14001/ certified.
Mineral Fibre 20 - 60 %
Cellulose Fibre 0 - 10 %
No direct contact of workers with clay (except sample
Clay 20 - 50 %
taking), as the clay is stored in a silo from where it
Perlite 10- 50 % automatically goes to a mixing tank after which the
Other < 1 % slurry is pumped to a holding tank.
Dispersion paint and mineral coatings are additionally
used for the surface finish as well as water during the 2.8 Product processing/Installation
production process.
There are no recognized systemic hazards associated
Contains substances on the /candidate list/ (date: with installing ceiling panels. Armstrong Building
16.07.2019) exceeding 0.1 mass percentage in at least Products recommends that installers handle materials
one partial product: no. in a manner to minimise airborne dust. Installers
should wear appropriate personal protective
Contains other Carcinogenic Mutagenic Reprotoxic equipment, such as gloves, safety glasses, and dust
(CMR) substances in categories 1A or 1B which are mask, to minimize exposure to dust and the potential
not on the /candidate list/, exceeding 0.1 mass for skin irritation.
percentage in at least one partial product: no.
2.9 Packaging
Flame retardants are not used. Thiadiazinanes
(“Dazomet”, an organosulfur compound) based The products are packed in cardboard cartons and
products are used as biocides. sealed with polyethene film. These cartons are then
stacked on chemically untreated wooden pallets which
are then wrapped with polyethene stretch film. Film,
paper and wood can be recycled in the usual way.
2.6 Manufacture
2.10 Condition of use
The described mineral products are produced using
the wet-felt process. The initial materials are mixed When used properly, the mineral products maintain
with water to a homogenous suspension that is then their mechanical and physical properties for their entire
pumped onto a belt conveyor (Fourdrinier). The water useful life.
is removed both mechanically (gravity and vacuum)
and by evaporation in a drying oven. The process 2.11 Environment and health during use
water is reused as much as possible. It is treated and
re-fed into the process water circuit. Production waste When correctly installed no dust / particles will be
and dust are reused in the production process. released during the period of use. The limits for
Armstrong World Industries is /ISO 9001/ certified. formaldehyde, VOC´s and Total Volatile Organic
Compound (TVOC)´s are in compliance with /DIN
2.7 Environment and health during 18177/
manufacturing
2.12 Reference service life
Armstrong World Industries meet EU and Germany
specific legal requirements for the production of The useful life of the mineral products is up to 50 years
mineral boards. depending on application, loading and level of
 It is prohibited to produce and use maintenance.
biopersistent fibres /Hazardous Substances
Ordinance (Annex iv, nr 22)
 It is prohibited to bring bio-persistent fibres
2.13 Extraordinary effects
onto the market /Chemicals Prohibition
Ordinance/ (Nr. 23 of the Annex to §1)
Fire
 Not subject to registration according to Article
7 or communication and notification according The declared products have the building material class
to Article 33 of the Regulation (EC) No A2-s1,d0 according to /EN 13501-1/. They are
therefore designated by German building regulations
1907/2006 of the European Parliament and of
as “non-combustible” with negligible smoke
the Council on the Registration, Evaluation,
development and no burning droplets in the case of
Authorisation and Restriction of Chemicals
fire.
(/REACH/) .
3 Environmental Product Declaration Armstrong World Industries Ltd – Ultima+ planks (19mm)
Fire protection 2.14 Re-use phase
Correctly demounted tiles and planks can be
Name Value reinstalled. Mineral tiles and planks can be returned to
Building material class A2 the production process for recycling into new mineral
Burning droplets s1 ceiling tiles when material separation and sufficient
Smoke gas development d0 material quality is available. Refer to Armstrong’s
recycling programme described under
Water www.armstrongceilings.com > “Corporate Social
Responsibility” > “Sustainability” > “Circular Economy”.
Prolonged contact with water dissolves the binding
starch which can lead to a loss of structure. Should the 2.15 Disposal
soluble components be carried into the sewage system
they are biodegradable, increasing Chemical Oxygen The /European Waste Code/ for site waste is
Demand (COD) and Biochemical Oxygen Demand designated as 17 09 04 and end-of-life and off-cut
(BOD) ceiling products can be returned to Armstrong for
recycling.
Mechanical destruction
2.16 Further information
If not handled correctly the surface and edges may be
broken or damaged. Additional information is available from the Armstrong
websites www.armstrongceilings.com
3. LCA: Calculation rules
3.1 Declared Unit  C1: Deconstruction (0 emissions as is done
by manual labour)
The declared unit for this EPD is 1m2 of Ultima+
 C2: Transportation to landfill (assumed to be
Planks (19mm) ceiling panel for use over 50 years
100 km)
Declared unit  C3: Waste processing (0 emissions)
 C4: End of life includes disposal of ceiling
panel (54.5% landfill, 44.5% incineration and
Name Value Unit 1% recycled)
Declared unit 1 m2
 D: Benefits and loads beyond the system
Grammage 5.5 kg/m2
boundary
Thickness of the panels 19 mm
Conversion factor to 1 kg 5.5 -
The Assessment Excludes:
 Steel suspension systems that are used for
most installations
 Overhead energy usage (heating, the lighting
3.2 System boundary
of manufacturing facility)
The system boundaries studied as part of this cradle to
grave LCA include the following information modules
as per /EN15804/ 3.3 Estimates and assumptions
The Cradle to Grave Assessment Includes: There are no specific assumptions to list that are not
 A1: Raw materials production including dealt with in the appropriate section.
substrate, coating, and packaging materials
for ceiling panels
3.4 Cut-off criteria
 A2: Transportation of raw materials to
Armstrong manufacturing facility
All inputs to a unit process that contribute to more than
 A3: Manufacturing of the ceiling panels at an 1% of the total mass or primary energy usage were
Armstrong facility included in the study.
 A3: Packaging of finished product including
It can be assumed that the total of neglected input
energy to operate packaging equipment
flows per module contributed to less than 5% of energy
 A4: Transportation from manufacturing facility
usage and mass.
to distribution centers, retailers, job site
(assumed to be 1200 km)
 A5: Installation into the building including 7% 3.5 Background data
construction waste.
The primary data for the ceiling tile manufacturing
 B1-7: Use and maintenance (0 emissions as
process was provided for the Munster manufacturing
the ceiling tiles do not require maintenance
facility for the year of 2016. The background data were
during life)
4 Environmental Product Declaration Armstrong World Industries Ltd – Ultima+ planks (19mm)
taken from the /Ecoinvent 3.3/ database and results Credits for electricity and heat gained from thermal
were calculated with /SimaPro 9.0/ software. recycling of waste and packaging in a solid waste
incinerator and/or landfill were included in this study
assuming an R1-value of below 60% (16% electrical
3.6 Data quality efficiency; 36% thermal efficiency).
To model the life cycle of the production of mineral 3.9 Comparability
boards, data was used which was collected from the Basically, a comparison or an evaluation of EPD data
Munster Germany manufacturing plant for the 2016 is only possible if all the data sets to be compared
production year. All other relevant data was taken were created according to EN 15804 and the building
from the /Ecoinvent 3.3/ database and is less than 10 context, respectively the product-specific
years old. characteristics of performance, are taken into account.
3.7 Period under review .
The data is representative of the manufacturing
processes of 2016.
3.8 Allocation
Energy (electrical and thermal from natural gas)
needed for the production at Armstrong has been
allocated by dividing the full energy consumption in
2016 by the total amount of ceiling tiles produced in
m2.
4. LCA: Scenarios and additional technical information
The following technical information is the basis for the assesse
declared modules or can be used for the development d (*)
of specific scenarios in the context of building Not
assessment. VOC in the air assesse kg
d (*)
Transport to the building site (A4)
(*) Note, measures for safe handling and installation
referred to in section 2.8 above.
Name Value Unit
Litres of fuel based on Ecoinvent Use or applicaiton of the installed product (B1-B7)
"market for transport, freight, lorry, 39.71 l/100km The use period for this product was considered as part
unspecified GLO" of the study. The reference service life (RSL) was 50
Transport distance 1200 km years. During this time period there is typically no
Capacity utilisation (including empty repair or maintenance that is required over any
50 %
runs) particular time period. The ceiling tile can typically last
Gross density of products transported 289 kg/m3 for the entire life of the building and there is no
Capacity utilisation volume factor 1 - recommended or generally accepted replacement or
refurbishment cycle. Once the ceiling tiles are in place
Installation into the building (A5) they do not require any energy or water usage.
Therefore the environmental impact of a ceiling tile
There is no energy or water use required for the ceiling during the use phase is negligible. All tiles meet VOC
tile installation. For suspended ceilings, a 7% waste test criteria as outlined in Section 7.
factor was assumed on-site during construction. This
value is based on historic internal studies which have
documented the quantity of scrap that is generated at
the job site due to needed cuts (to allow for installation
of sprinkler heads, for example) or mistakes. While
this material can be and is recycled from some jobs, it
is assumed that all of the on-site scrap material will be
Reference service life
sent off-site for disposal.
Name Value Unit
Reference service life 50 a
Name Value Unit
Auxiliary 0 kg
End of life (C1-C4)
Water consumption 0 m3
C1 and C3 have been estimated to be zero. As a
Other resources 0 kg
consequence, an impact of zero resulted for all results
Electricity consumption 0 kWh
indicators assessed for these modules. For this study,
Other energy carriers 0 MJ
54,5% ceiling tiles that are not recycled are sent to
Material loss 0.385 kg
landfill and 44,5% are incinerated. Despite that
Output substances following waste
0 kg Armstrong has a recycling programme in place, the
treatment on site
recycling rate of ceiling tiles at End of Life (EoL) is
Dust in the air Not kg
estimated at 1%. As a consequence of this very low
5 Environmental Product Declaration Armstrong World Industries Ltd – Ultima+ planks (19mm)
recycling rate, loads and benefits beyond the system
boundary from recycling the product itself at EoL have
been estimated to be zero (total results for module D
however are not zero due to contributions from other
phases, such as production).
Name Value Unit
Collected separately 0 kg
Collected as mixed construction waste 5.8 kg
Reuse 0 kg
Recycling 0.06 kg
Landfilling 3.2 kg
Energy recovery 0 kg
Distance to incinerator or landfill 100 km
R1 factor for Waste incineration <60 %
Thermal treatment (EoL incineration) 2.6 kg
Reuse, recovery and/or recycling potentials (D),
relevant scenario information
In module D reuse of the wooden pallet (98%), avoided
electricity and heat production because of thermal
treatment are accounted for, as well as the loss of
stone wool and glass fibre (99% landfill or thermally
treated) that entered the system as secondary
materials.
6 Environmental Product Declaration Armstrong World Industries Ltd – Ultima+ planks (19mm)
5. LCA: Results
DESCRIPTION OF THE SYSTEM BOUNDARY (X = INCLUDED IN LCA; MND = MODULE NOT DECLARED;
MNR = MODULE NOT RELEVANT)
BENEFITS AND
CONSTRUCTI LOADS
PRODUCT STAGE ON PROCESS USE STAGE END OF LIFE STAGE BEYOND THE
STAGE SYSTEM
BOUNDARIES
7 Environmental Product Declaration Armstrong World Industries Ltd – Ultima+ planks (19mm)
lairetam
waR
ylppus tropsnarT
gnirutcafunaM
eht
morf
tropsnarT
etis
eht
ot
etag
ylbmessA esU
ecnanetniaM
riapeR
tnemecalpeR tnemhsibrufeR
ygrene
lanoitarepO esu
retaw
lanoitarepO esu
noitcurtsnoc-eD
noitilomed tropsnarT
gnissecorp
etsaW
lasopsiD -esueR -yrevoceR -gnilcyceR laitnetop
A1 A2 A3 A4 A5 B1 B2 B3 B4 B5 B6 B7 C1 C2 C3 C4 D
X X X X X X X X X X X X X X X X X
RESULTS OF THE LCA - ENVIRONMENTAL IMPACT according to EN 15804+A1: 1 m² Ultima+ Planks
(19mm)
Parameter Unit A1-A3 A4 A5 B1 B2 B3 B4 B5 B6 B7 C1 C2 C3 C4 D
8.33E+ 0.00E+ 0.00E+ 0.00E+ 0.00E+ 0.00E+ 0.00E+ 0.00E+ 0.00E+ 0.00E+ -1.63E-
GWP [kg CO2-Eq.]
0
8.73E-16.07E-1
0 0 0 0 0 0 0 0
8.07E-2
0
1.40E-1
1
0.00E+ 0.00E+ 0.00E+ 0.00E+ 0.00E+ 0.00E+ 0.00E+ 0.00E+ 0.00E+ -5.19E-
ODP [kg CFC11-Eq.] 8.11E-71.63E-75.91E-8 1.50E-8 1.41E-8
0 0 0 0 0 0 0 0 0 8
0.00E+ 0.00E+ 0.00E+ 0.00E+ 0.00E+ 0.00E+ 0.00E+ 0.00E+ 0.00E+ -1.09E-
AP [kg SO2-Eq.] 3.79E-23.84E-32.76E-3
0 0 0 0 0 0 0 0
3.55E-4
0
3.92E-4
3
0.00E+ 0.00E+ 0.00E+ 0.00E+ 0.00E+ 0.00E+ 0.00E+ 0.00E+ 0.00E+ -2.56E-
EP [kg (PO4)3--Eq.] 6.32E-36.95E-44.66E-4
0 0 0 0 0 0 0 0
6.43E-5
0
7.55E-5
4
0.00E+ 0.00E+ 0.00E+ 0.00E+ 0.00E+ 0.00E+ 0.00E+ 0.00E+ 0.00E+ -7.81E-
POCP [kg ethene-Eq.] 2.12E-31.55E-41.54E-4 1.44E-5 2.87E-5
0 0 0 0 0 0 0 0 0 5
0.00E+ 0.00E+ 0.00E+ 0.00E+ 0.00E+ 0.00E+ 0.00E+ 0.00E+ 0.00E+ -2.57E-
ADPE [kg Sb-Eq.] 1.12E-52.46E-68.09E-7 2.28E-7 1.12E-7
0 0 0 0 0 0 0 0 0 7
-
9.35E+ 1.32E+ 6.74E+ 0.00E+ 0.00E+ 0.00E+ 0.00E+ 0.00E+ 0.00E+ 0.00E+ 0.00E+ 1.23E+ 0.00E+ 1.28E+
ADPF [MJ] 2.10E+
1 1 0 0 0 0 0 0 0 0 0 0 0 0
0
GWP = Global warming potential; ODP = Depletion potential of the stratospheric ozone layer; AP = Acidification potential of land and water; EP =
Caption Eutrophication potential; POCP = Formation potential of tropospheric ozone photochemical oxidants; ADPE = Abiotic depletion potential for non-
fossil resources; ADPF = Abiotic depletion potential for fossil resources
RESULTS OF THE LCA - RESOURCE USE according to EN 15804+A1: 1 m² Ultima+ Planks (19mm)
Parameter Unit A1-A3 A4 A5 B1 B2 B3 B4 B5 B6 B7 C1 C2 C3 C4 D
PERE [MJ] 7.69E+0 1.85E-1 5.43E-1 0.00E+00.00E+00.00E+00.00E+00.00E+00.00E+00.00E+00.00E+0 1.71E-2 0.00E+0 3.52E-2-9.07E+0
PERM [MJ] 1.04E+10.00E+0 7.28E-1 0.00E+00.00E+00.00E+00.00E+00.00E+00.00E+00.00E+00.00E+00.00E+00.00E+00.00E+00.00E+0
PERT [MJ] 1.81E+1 1.85E-1 1.27E+00.00E+00.00E+00.00E+00.00E+00.00E+00.00E+00.00E+00.00E+0 1.71E-2 0.00E+0 3.52E-2-9.07E+0
PENRE [MJ] 1.15E+21.43E+18.27E+00.00E+00.00E+00.00E+00.00E+00.00E+00.00E+00.00E+00.00E+01.33E+00.00E+01.39E+0-2.49E+0
PENRM [MJ] 2.27E+00.00E+0 1.59E-1 0.00E+00.00E+00.00E+00.00E+00.00E+00.00E+00.00E+00.00E+00.00E+00.00E+00.00E+00.00E+0
PENRT [MJ] 1.17E+21.43E+18.43E+00.00E+00.00E+00.00E+00.00E+00.00E+00.00E+00.00E+00.00E+01.33E+00.00E+01.39E+0-2.49E+0
SM [kg] 0.00E+00.00E+00.00E+00.00E+00.00E+00.00E+00.00E+00.00E+00.00E+00.00E+00.00E+00.00E+00.00E+00.00E+00.00E+0
RSF [MJ] IND IND IND IND IND IND IND IND IND IND IND IND IND IND IND
NRSF [MJ] IND IND IND IND IND IND IND IND IND IND IND IND IND IND IND
FW [m³] 4.58E-2 2.62E-3 3.38E-3 0.00E+00.00E+00.00E+00.00E+00.00E+00.00E+00.00E+00.00E+0 2.42E-4 0.00E+0 4.96E-4-9.31E-4
PERE = Use of renewable primary energy excluding renewable primary energy resources used as raw materials; PERM = Use of
renewable primary energy resources used as raw materials; PERT = Total use of renewable primary energy resources; PENRE = Use of
non-renewable primary energy excluding non-renewable primary energy resources used as raw materials; PENRM = Use of non-
Caption
renewable primary energy resources used as raw materials; PENRT = Total use of non-renewable primary energy resources; SM = Use
of secondary material; RSF = Use of renewable secondary fuels; NRSF = Use of non-renewable secondary fuels; FW = Use of net fresh
water
RESULTS OF THE LCA – OUTPUT FLOWS AND WASTE CATEGORIES according to EN 15804+A1:
1 m² Ultima+ Planks (19mm)
Parameter Unit A1-A3 A4 A5 B1 B2 B3 B4 B5 B6 B7 C1 C2 C3 C4 D
HWD [kg] 1.34E-4 8.05E-6 9.57E-6 0.00E+00.00E+00.00E+00.00E+00.00E+00.00E+00.00E+00.00E+0 7.45E-7 0.00E+0 1.26E-6-1.53E-5
NHWD [kg] 1.06E+0 8.19E-1 2.93E-1 0.00E+00.00E+00.00E+00.00E+00.00E+00.00E+00.00E+00.00E+0 7.57E-2 0.00E+03.02E+0-2.25E-2
RWD [kg] 3.35E-4 9.25E-5 2.47E-5 0.00E+00.00E+00.00E+00.00E+00.00E+00.00E+00.00E+00.00E+0 8.55E-6 0.00E+0 7.88E-6-7.20E-6
CRU [kg] 0.00E+00.00E+01.41E+00.00E+00.00E+00.00E+00.00E+00.00E+00.00E+00.00E+00.00E+00.00E+00.00E+00.00E+00.00E+0
MFR [kg] 0.00E+00.00E+0 7.90E-3 0.00E+00.00E+00.00E+00.00E+00.00E+00.00E+00.00E+00.00E+00.00E+00.00E+0 1.12E-1 0.00E+0
MER [kg] 0.00E+00.00E+04.27E+00.00E+00.00E+00.00E+00.00E+00.00E+00.00E+00.00E+00.00E+00.00E+00.00E+00.00E+00.00E+0
EEE [MJ] 0.00E+00.00E+01.27E+10.00E+00.00E+00.00E+00.00E+00.00E+00.00E+00.00E+00.00E+00.00E+00.00E+04.14E+10.00E+0
EET [MJ] 0.00E+00.00E+02.13E+10.00E+00.00E+00.00E+00.00E+00.00E+00.00E+00.00E+00.00E+00.00E+00.00E+07.13E+10.00E+0
HWD = Hazardous waste disposed; NHWD = Non-hazardous waste disposed; RWD = Radioactive waste disposed; CRU = Components
Caption for re-use; MFR = Materials for recycling; MER = Materials for energy recovery; EEE = Exported electrical energy; EEE = Exported
thermal energy
6. LCA: Interpretation
As process phase A1-A3 contributes most, the major
contributions within this process phase have been
further analysed and presented below. The graph
shows that major contributions originate from heat
production from natural gas at the production site of
Armstrong (dark blue; combustion emissions), the
production of stone wool (light orange; direct emissions
from production), maize starch production (light blue;
maize cultivation and infrastructure for processing) and
electricity usage (light grey; major contributor in the
electricity mix for Germany is electricity generated by
burning brown coal).
The graph shows the individual contributions of the
process phases to each environmental impact included
in the LCA of the Ultima+ Planks 19mm Ceiling
Tile. The graph clearly shows that the module A1-A3
contributes most to the environmental impact of all
impact categories. Module D has a negative
contribution, which is caused by energy recovery from
incineration in the end-of-life stage. There is no
secondary material used in this product and therefore
no impact is calculated for the loss of secondary
material in module D.
7. Requisite evidence
7.1 Biopersistence AgBB Overview (28 Days)
Verification of fulfilment of the requirements of annexe The limits according to the /AgBB scheme/ are
IV, Nr. 22 of the /Hazardous Substances Ordinance/ adhered to
and section 23 of the appendix to § 1 /Chemicals
Prohibition Ordinance/ is provided by the RAL quality Name Value Unit
mark 388 or individual evidence. The following half-life TVOC (C6 - C16) 1000 μg/m3
periods were calculated according to EU protocol: Sum SVOC (C16 - C22) 100 μg/m3
WHO filament fibre (L > 5 μm, D < 3 μm, L/D> 3/1): ≤ R (dimensionless) 1 -
40 days long filament fibre (length > 20 μm, L/D>3/1): VOC without NIK 100 μg/m3
< 40 days Carcinogenic Substances 1 μg/m3
Test body: Fraunhofer Institute for Toxicology and Test body: ITB, Poland; Certificate
Experimental Medicine, 30625 Hanover. ITEM / ITA no. 01398/13/Z00NF (07-2013).
study no. 02G1307 (10-Jul-2014) / 02G04001 (08-Aug-
2007)
7.3 Radioactivity
Radioactivity is not relevant for our products
7.2 Formaldehyde and VOC emissions
8. References
/AgBB scheme/: Committee for Health-related preparations and products according to the Chemicals
Evaluation of Building Products (Ausschuss zur Act.
gesundheitlichen Bewertung von Bauprodukten –
AgBB), Health-related Evaluation of Emissions of /Commission Decision on the European List of
Volatile Organic Compounds (VVOC, VOC and SVOC) Waste/: COM 2000/532/EC.
from Building Products.
/DIN 18177/: DIN 18177: 2012-11, Wet felt factory-
/CEN - EN 717-1/: Wood based panels - Determination produced mineral panels - Characteristics and test
of formaldehyde release - Part 1: Formaldehyde methods.
emission by the chamber method.
/Ecoinvent 3.3/: Originally released August 2016,
/Chemicals Prohibition Ordinance/: (Nr. 23 of the implemented in SimaPro, PRé Sustainability,
Annex to §1): Ordinance on bans and restrictive December 2016.
measures for the marketing of hazardous substances,
8 Environmental Product Declaration Armstrong World Industries Ltd – Ultima+ planks (19mm)
/EN 13501-1/: EN 13501-1:2007, Fire classification of
construction products and building elements - Part 1: /IBU, 2018 PCR Part-A v1.7/: Calculation Rules for the
Classification using data from reaction to fire tests. Life Cycle Assessment and Requirements on the
Project Report.
/EN 13964/: EN 13964: 2014, Suspended ceilings -
Requirements and test methods. /IBU, 2017 PCR Part-B v1.6/: Requirements on the
EPD for Mineral panels”.
/EN 15804/: EN 15804:2012+A1:2014, Sustainability
of construction works - Environmental product /ISO 14001/: ISO 14001: 2015, Environmental
declarations - Core rules for the product category of management systems - Requirements with guidance
construction products. for use.
/EN ISO 10848-2/: EN ISO 10848-2: 2006, Acoustics - /ISO 14040/: ISO 14040: 2006, Environmental
Laboratory measurement of the flanking transmission management. Life cycle assessment - Principles and
of airborne and impact sound between adjoining framework.
rooms.
/ISO 14044/: ISO 14044: 2006, Environmental
/EN ISO 11654/: EN ISO 11654: 1997, Acoustics - management. Life cycle assessment – Requirements
Sound absorbers for use in buildings - Rating of sound and Guidelines.
absorption.
/ISO 21930/: ISO 21930: 2017, Sustainability in
/EN ISO 11654/: EN ISO 11654: 1997, Acoustics — building construction -- Environmental declaration of
Sound absorbers for use in buildings — Rating of building products.
sound absorption.
/ISO 9001/: ISO 9001: 2015, Quality management
/EN ISO 354/: EN ISO 354: 2003, Acoustics - systems - Requirements.
Measurement of sound absorption in a reverberation
room. /RAL quality mark 388/: Products made of mineral
wool.
/EN ISO 717-1/: EN ISO 717-1: 2013, Acoustics -
Rating of sound insulation in buildings and of building Regulation (EC) No 1907/2006/: of the European
elements - Part 1: Airborne sound insulation. Parliament and of the Council of 18 December 2006
concerning the Registration, Evaluation, Authorisation
European Chemicals Agency (ECHA)/: Candidate and Restriction of Chemicals (REACH).
List/ of Substances of Very High Concern (SVHC) for
Authorisation: https://echa.europa.eu/candidate-list- /Regulation (EU) No. 305/2011 (CPR)/: European
table (date: 16.07.2019; 201 substances listed). regulation of 9 March 2011 that lays down harmonised
conditions for the marketing of construction products.
/European Waste Code/: European Waste Code 17
09 04, Mixed construction and demolition wastes other /SimaPro 9.0/: PRé Sustainability, Amersfoort, The
than those mentioned in 17 09 01, 17 09 02 and 17 09 Netherlands, 2019.
03.
/Formaldehyde and VOC emissions/: Product
emission test with AgBB/DIBt test protocol.
/Hazardous Substances Ordinance/: (Annex iv, nr
22): Ordinance on the protection against hazardous
substances.
9 Environmental Product Declaration Armstrong World Industries Ltd – Ultima+ planks (19mm)
Publisher
Institut Bauen und Umwelt e.V. Tel +49 (0)30 3087748- 0
Panoramastr. 1 Fax +49 (0)30 3087748- 29
10178 Berlin Mail info@ibu-epd.com
Germany Web www.ibu-epd.com
Programme holder
Institut Bauen und Umwelt e.V. Tel +49 (0)30 - 3087748- 0
Panoramastr 1 Fax +49 (0)30 – 3087748 - 29
10178 Berlin Mail info@ibu-epd.com
Germany Web www.ibu-epd.com
Author of the Life Cycle
Assessment Tel +31 882 146 600
SGS Search Fax +31 (0)20 506 16 17
Petroleumhavenweg 8 Mail harry.vanewijk@sgs.com
1041 AC Amsterdam Web www.sgssearch.nl
Netherlands
Owner of the Declaration
Armstrong World Industries Ltd Tel +44 (0) 1895 910022
Kingsway South/Team Valley Fax -
Trading Estate 0108 Mail
11 OSP Gateshead Tyne & Wear iclarke@armstrongceilingsolution
Netherlands s.co.uk
Web www.armstrongceilings.com
