ENVIRONMENTAL PRODUCT DECLARATION
as per ISO 14025 and EN 15804+A2
Owner of the Declaration Knauf Ceiling Solutions GmbH & Co. KG
Publisher Institut Bauen und Umwelt e.V. (IBU)
Programme holder Institut Bauen und Umwelt e.V. (IBU)
Declaration number EPD-KNA-20240278-IBA1-EN
Issue date 26/11/2024
Valid to 25/11/2029
ADAGIO HD+ (35 mm)
Knauf Ceiling Solutions GmbH & Co. KG
www.ibu-epd.com | https://epd-online.com
1. General Information
Knauf Ceiling Solutions GmbH & Co. KG ADAGIO HD+ (35 mm)
Programme holder Owner of the declaration
IBU – Institut Bauen und Umwelt e.V. Knauf Ceiling Solutions GmbH & Co. KG
Hegelplatz 1 Elsenthal 15
10117 Berlin 94481 Grafenau
Germany Germany
Declaration number Declared product / declared unit
EPD-KNA-20240278-IBA1-EN 1 m² ADAGIO HD+ mineral ceiling tiles with a surface weight of 9.49 kg/m².
This declaration is based on the product category rules: Scope:
Mineral panels, 01/08/2021 This document refers to 1 m² ADAGIO HD+ mineral ceiling tiles with a
(PCR checked and approved by the SVR) surface weight of 9.49 kg/m² and a thickness of 35 mm, manufactured at
the production facility in Grafenau, Germany.
Issue date The owner of the declaration shall be liable for the underlying information
and evidence; the IBU shall not be liable with respect to manufacturer
26/11/2024
information, life cycle assessment data and evidences.
The EPD was created according to the specifications of EN 15804+A2. In
Valid to
the following, the standard will be simplified as EN 15804.
25/11/2029
Verification
The standard EN 15804 serves as the core PCR
Independent verification of the declaration and data according to ISO
14025:2011
internally X externally
Dipl.-Ing. Hans Peters
(Chairman of Institut Bauen und Umwelt e.V.)
Florian Pronold Dr.-Ing. Nikolay Minkov,
(Managing Director Institut Bauen und Umwelt e.V.) (Independent verifier)
1 Environmental Product Declaration - Knauf Ceiling Solutions GmbH & Co. KG - ADAGIO HD+ (35 mm)
2. Product
2.1 Product description/Product definition This product/article/at least one partial article contains
The ceiling tiles are manufactured using a wet-felt process and substances listed in the ECHA-candidate list (date: 25.06.2020)
consist of biosoluble mineral wool, perlite, clay and starch. The exceeding 0.1 percentage by mass: No
ceiling tiles meet the requirements of DIN 18177 and DIN EN
13964. This product/article/at least one partial article contains other
carcinogenic, mutagenic, reprotoxic (CMR) substances in
The mineral tiles are available in a wide range of different categories 1A or 1B which are not on the candidate list,
surface designs and product properties. Depending on the exceeding 0.1 percentage by mass: No
design, the ceiling tiles are available in different formats and
edge finishes. Biocide products were added to this construction product or it
has been treated with biocide products (this then concerns a
This EPD applies to the following products: treated product as defined by the (EU) Ordinance on Biocide
ADAGIO HD+ (35 mm) Products No. 528/2012): No
For the placing on the market of the product in the European In-can preservatives are used in the production process;
Union/European Free Trade Association (EU/EFTA) (with the however, they are not part of the products and are therefore not
exception of Switzerland) Regulation (EU) No. 305/2011 (CPR) within the scope of the Ordinance on Biocide Products.
applies. The product needs a declaration of performance taking
into consideration EN 13964:2014, suspended ceiling 2.6 Manufacture
requirements and test methods and the CE-marking. For the The mineral tiles are produced in the traditional wet process
application and use the respective national provisions apply. (wet-felt). The raw materials are mixed with water to form a
homogeneous suspension, which is pumped onto a belt
2.2 Application conveyor (Fourdrinier). The water is removed mechanically
Mineral tiles (wet-felt) are typically used as lay in for suspended (gravity and vacuum) and by evaporation in the drying oven. As
ceiling constructions. They are primarily used as optical far as possible, the process water is reused. It is treated
cladding, but also for sound absorption and sound insulation, accordingly and fed back into the process water circuit.
for fire resistance and against fire spreading, for cleanrooms Depending on the desired appearance the panels can be
and high hygiene requirements. sanded, colour-treated, patterned, eroded or embossed.
Production waste and dust are reused in the process in the
2.3 Technical Data
sense of an internal cycle.
Mineral boards (wet-felt) are regulated by EN 13964 and have The manufacturing plant is certified according to ISO 9001, ISO
corresponding labelling and declaration of performance. The 14001, ISO 45001 and ISO 50001.
following data provide an overview of results:
2.7 Environment and health during manufacturing
Construction data (according to DIN 18177)
The manufacturer complies with the special German and
Name Value Unit
European regulations for the production of mineral slabs:
Thermal conductivity 0.06 W/(mK)
• The manufacturing plant is certified according to ISO
Sound absorption coefficient acc. ISO 354 and
0.9 % 9001, ISO 14001, ISO 45001 and ISO 50001.
ISO 11654
• The production has a closed water cycle.
Airborne sound reduction acc. ISO 10848 and
43 dB • Production generates almost no waste, resulting blanks,
EN 717-1
dust and rejects are reused.
Gross density 271 kg/m3 • Exclusive use of mineral fibres according to Regulation
(EU) No.1272/2008 Note Q.
Performance data of the product in accordance with the
• Prohibition of the production and use of biopersistent
declaration of performance with respect to its essential
fibres (Ordinance on Hazardous Substances, Annex II,
characteristics according to EN 13964:2014, suspended ceiling
No. 5).
requirements and test methods (not part of CE-marking).
• Prohibition of placing biopersistent fibres on the market
2.4 Delivery status (Chemicals Prohibition Order, No.23 of the Annex to
§1).
The EPD refers to ADAGIO HD+ 35 mm which can have
• Not subject to declaration according to REACH.
variable length and width dimensions.
2.8 Product processing/Installation
2.5 Base materials/Ancillary materials
There are no recognised systemic hazards associated with the
Mineral tile composition:
installation of ceiling tiles. It is recommended that materials are
Name Value Unit handled in a manner that minimises dust generation. Workers
Mineral wool 55 - 60 % should wear appropriate personal protective equipment.
Equipment such as gloves, goggles and dust masks are
Clay 10 - 15 %
recommended to minimise exposure to dust and prevent skin
Cellulose fibres 0 - 5 %
irritation.
Starch 5 - 10 %
others 0 - 15 % 2.9 Packaging
Brokes / Dust 5 - 10 % The panels are packaged with cardboard boxes and sealed
with transparent polyethylene film. These packages lie on
In addition, dispersion paints are used on the surface and water
chemically untreated wooden pallets. The pallets are wrapped
for preparation during production. The recycled content is
with polyethylene stretch film. Foil, paper and wood can be
49.4 %.
recycled in the usual ways.
2 Environmental Product Declaration - Knauf Ceiling Solutions GmbH & Co. KG - ADAGIO HD+ (35 mm)
2.10 Condition of use Water
When handled properly, the mechanical and structural-physical In the case of prolonged contact with water, the starch binder
properties of the mineral tile remain intact throughout its entire dissolves, which can lead to a loss of structure, and if the
service life. Direct contact with water should be avoided due to soluble components are discharged into the sewage treatment
the water-soluble binding agent starch. plant, they are biodegradable, increasing the chemical oxygen
demand (COD) and the biological oxygen demand (BOD).
2.11 Environment and health during use
When properly installed, no dust/particles are released during Mechanical destruction
the use phase. For the substance groups formaldehyde, volatile The mineral slabs (wet-felt) can be broken by hand and also
organic compounds (VOCs) and total volatile organic damaged superficially, which can result in minor dust formation.
compounds (TVOCs), the limits according to DIN 18177 are
complied with. 2.14 Re-use phase
If the panels are removed properly, they can be reinstalled. In
2.12 Reference service life
case of minor damage, the slabs can be reused as cut-to-size
The service life of the mineral tiles (wet-felted) is up to 50 tiles. Mineral tiles can be returned to the manufacturing process
years, depending on the area of use, exposure and state of if they are of the correct type and have sufficient material
maintenance. Within the framework of the conditions of use, no quality; they can be recycled up to 100 %.
ageing effects are to be expected apart from visual
discolouration caused by air circulation. 2.15 Disposal
The waste code number of production residues for mineral tiles
2.13 Extraordinary effects
according to the AVV, German List of Wastes Ordinance is 10
Fire 11 03, the waste code number for construction site waste
The declared products are classified in the fire reaction class (offcuts) is 17 06 04. If the tiles are not recycled as described in
A2-s1, d0 according to EN 13501-1. This means that they are 2.14., they are disposed of in a landfill.
"non-combustible" according to the German building authority
designation (and also many other European countries) with 2.16 Further information
negligible smoke development and no burning drip in the event Further information at www.knaufceilingsolutions.com
of fire.
Fire Reaction
Name Value
Building material class A2
Smoke gas development s1
Burning droplets d0
3. LCA: Calculation rules
German power grid (considered based on the German residual
3.1 Declared Unit mix) and thermal energy from natural gas. Also, the packaging
This EPD refers to a declared unit of 1 m² ADAGIO HD+ of the products is considered.
mineral ceiling tiles with a surface weight of 9.49 kg/m² and a
thickness of 35 mm. Module C1 | Deconstruction and demolition
Declared Unit Disassembly of the product is done either manually or using
smaller tools. Referring energy demand is considered to be
Name Value Unit
negligible.
Declared unit 1 m2
Grammage 9.49 kg/m2 Modul C2 | Transport to disposal
Layer thickness 0.035 m The transport to the disposal of the material is estimated
declaring a 50 km radius to the landfill. In reality, this scenario
The ceiling tiles are produced at the Knauf Ceiling Solutions
may vary depending on the actual location of deconstruction
production site in Grafenau, Germany.
and referring waste treatment.
As the declaration refers to a specific product, no averages had
Module C3 | Waste processing
to be calculated.
The declared scenario assumes landfilling of the product.
Referring environmental impacts are accounted for in module
3.2 System boundary
C4.
The life cycle assessment of ADAGIO HD+ mineral ceiling tiles
includes a cradle-to-gate analysis of the products'
Module C4 | Disposal
environmental impacts with modules C1–C4 and module D
Module C4 refers to the emissions from the disposal of the
(A1–A3, + C + D). Subsequent life cycle phases are part of the
mineral ceiling tiles. The chosen scenario, therefore, includes
analysis:
the environmental burdens of landfilling of the product.
Module A1–A3 | Production stage
Module D | Benefits and loads beyond the system
The production stage includes the upstream burdens of raw
boundary
material supply, their transports and the manufacturing plant of
The declared scenario assumes landfilling of the product.
Knauf Ceiling Solutions located in Grafenau (Germany). Mineral
Referring environmental impacts are accounted for in module
ceiling tiles are produced in the wet-felt process. Main raw
C4.
material inputs, therefore, refer to mineral wool, perlite, clay and
starch. The production site is supplied with electricity from the
3 Environmental Product Declaration - Knauf Ceiling Solutions GmbH & Co. KG - ADAGIO HD+ (35 mm)
datasets refer to the latest versions available and are carefully
3.3 Estimates and assumptions chosen.
Assumptions and approximations are applied in case of a lack
of representative data. All assumptions and approximations are 3.7 Period under review
documented precisely and represent a best-guess Foreground data were collected in the 2023 production year,
representation of reality. In case of uncertainty, a conservative and the data are based on the volumes produced on an annual
approach is chosen. basis.
3.4 Cut-off criteria 3.8 Geographic Representativeness
The LCA model covers all available input and output flows, Land or region, in which the declared product system is
which can be represented based on robust data. Data gaps are manufactured, used or handled at the end of the product´s
filled with conservative assumptions from average data (when lifespan: Germany
available) or with generic data and are documented
accordingly. Only data with a contribution lower 1 % were cut
3.9 Allocation
off. Thus, no data were neglected, of which a substantial impact
is to be expected. All relevant data were collected All information for the allocation of given material and energy
comprehensively. Cut-off material and energy flows were flows is based on the ERP-systems of the production site.
chosen carefully based on their expected quantitative Annual input quantities are only available for the overall
contribution as well as potential environmental impacts. Thus, it production site. Thus, the calculation of specific input quantities
can be assumed that the sum of all neglected input flows does for the raw board production is based on their respective
not account for more than 5 % of the total material, water and recipe. In addition, product specific application rates of
energy flows. backcoat and primer were available. The total annual energy
consumption as well as waste quantities were broken down to
3.5 Background data the product under study based on their production share
This study uses generic background data for the evaluation of (produced square meters).
upstream environmental impacts from MLC 2023.2 database in
the LCA FE-software version 10. Knauf Ceiling Solutions uses waste paper and waste fibre glass
as secondary material. Waste paper reaches its end of waste
3.6 Data quality status after sorting of the paper, waste fibre glass after sorting
Data collection is based on product-specific questionnaires. It and grinding. As a result, the upstream supply chain of waste
follows an iterative process clarifying questions via e-mail, paper and waste fibre glass are considered burden-free. The
telephone calls or in personal/web meetings. Intensive system boundary for secondary raw materials defined in EN
discussions between Knauf Ceiling Solutions and Daxner & 15804 applies.
Merl result in an accurate mapping of product-related material
and energy flows. This leads to a high quality of foreground 3.10 Comparability
data collected. Data collection relies on a consistent process Basically, a comparison or an evaluation of EPD data is only
according to ISO 14044. possible if all the data sets to be compared were created
according to EN 15804 and the building context, respectively
The technological, geographical and time-related the product-specific characteristics of performance, are taken
representativeness of the database was kept in mind when into account.
selecting background data. Whenever specific data were The MLC 2023.2 background database (former GaBi) in the
missing, either generic datasets or representative average data LCA FE-software version 10 was used to calculate the LCA.
were used instead. The implemented MLC background
4. LCA: Scenarios and additional technical information
A3.
Characteristic product properties of biogenic carbon
Assembly (A5)
The biogenic carbon content quantifies the amount of biogenic
The End-of-Life of the product packaging is not declared in
carbon in the declared product.
module A5.
Information on the description of the biogenic carbon
Name Value Unit
content at the factory gate
Packaging (cardboard) 0.086 kg/m²
Name ValueUnit
Packaging (pallets) 0.243 kg/m²
kg
Biogenic carbon content in product 0.28 Packaging (polyethylene foil) 0.025 kg/m²
C
Biogenic carbon content in accompanying kg
0.14
packaging C End-of-Life (C1–4)
Note: 1 kg of biogenic carbon is equivalent to 44/12 kg of CO 2. Name Value Unit
Collected separately waste type 9.49 kg
Landfilling 9.49 kg
As the End-of-Life of the product packaging is not declared in
module A5, its carbon uptake is not considered in module A1–
4 Environmental Product Declaration - Knauf Ceiling Solutions GmbH & Co. KG - ADAGIO HD+ (35 mm)
5. LCA: Results
The following table contains the LCA results for a declared unit of 1 m² ADAGIO HD+ mineral ceiling tiles with a surface weight of
9.49 kg/m² and a thickness of 35 mm.
DESCRIPTION OF THE SYSTEM BOUNDARY (X = INCLUDED IN LCA; MND = MODULE OR INDICATOR NOT DECLARED; MNR
= MODULE NOT RELEVANT)
Benefits and
Construction loads beyond
Product stage Use stage End of life stage
process stage the system
boundaries
la ire ta m w a Ry lp p u s tro p s n a rT g n iru tc a fu n a M e h t m o rf tro p s n a rTe tis e h t o t e ta g y lb m e s s A e s U e c n a n e tn ia M ria p e R tn e m e c a lp e R tn e m h s ib ru fe R y g re n e la n o ita re p Oe s u re ta w la n o ita re p Oe s u n o itc u rts n o c -e Dn o itilo m e d tro p s n a rT g n is s e c o rp e ts a W la s o p s iD -e s u e R-y re v o c e R-g n ilc y c e Rla itn e to p
A1 A2 A3 A4 A5 B1 B2 B3 B4 B5 B6 B7 C1 C2 C3 C4 D
X X X MND MND MND MND MNR MNR MNR MND MND X X X X X
RESULTS OF THE LCA - ENVIRONMENTAL IMPACT according to EN 15804+A2: 1 m² ADAGIO HD+ mineral ceiling tiles (9.49
kg/m²)
Parameter Unit A1-A3 C1 C2 C3 C4 D
Global Warming Potential total (GWP-total) kg CO 2 eq 7.4E+00 0 3.46E-02 0 1.17E+00 0
Global Warming Potential fossil fuels (GWP-fossil) kg CO 2 eq 8.94E+00 0 3.42E-02 0 1.4E-01 0
Global Warming Potential biogenic (GWP-biogenic) kg CO 2 eq -1.55E+00 0 7.82E-05 0 1.03E+00 0
Global Warming Potential luluc (GWP-luluc) kg CO 2 eq 5.18E-03 0 3.2E-04 0 4.43E-04 0
Depletion potential of the stratospheric ozone layer (ODP) kg CFC11 eq 2.12E-10 0 4.5E-15 0 3.62E-13 0
Acidification potential of land and water (AP) mol H+ eq 5.05E-02 0 1.23E-04 0 1.01E-03 0
Eutrophication potential aquatic freshwater (EP-freshwater) kg P eq 2.53E-04 0 1.26E-07 0 2.87E-07 0
Eutrophication potential aquatic marine (EP-marine) kg N eq 9.34E-03 0 5.62E-05 0 2.61E-04 0
Eutrophication potential terrestrial (EP-terrestrial) mol N eq 1.62E-01 0 6.31E-04 0 2.87E-03 0
Formation potential of tropospheric ozone photochemical oxidants kg NMVOC
1.7E-02 0 1.11E-04 0 7.88E-04 0
(POCP) eq
Abiotic depletion potential for non fossil resources (ADPE) kg Sb eq 1.41E-06 0 2.29E-09 0 6.59E-09 0
Abiotic depletion potential for fossil resources (ADPF) MJ 1.31E+02 0 4.71E-01 0 1.9E+00 0
m3 world eq
Water use (WDP) 3.52E+00 0 4.18E-04 0 1.56E-02 0
deprived
RESULTS OF THE LCA - INDICATORS TO DESCRIBE RESOURCE USE according to EN 15804+A2: 1 m² ADAGIO HD+ mineral
ceiling tiles (9.49 kg/m²)
Parameter Unit A1-A3 C1 C2 C3 C4 D
Renewable primary energy as energy carrier (PERE) MJ 2.97E+00 0 3.43E-02 0 3.09E-01 0
Renewable primary energy resources as material utilization
MJ 1.79E+01 0 0 0 0 0
(PERM)
Total use of renewable primary energy resources (PERT) MJ 2.09E+01 0 3.43E-02 0 3.09E-01 0
Non renewable primary energy as energy carrier (PENRE) MJ 1.31E+02 0 4.73E-01 0 1.9E+00 0
Non renewable primary energy as material utilization (PENRM) MJ 0 0 0 0 0 0
Total use of non renewable primary energy resources (PENRT) MJ 1.31E+02 0 4.73E-01 0 1.9E+00 0
Use of secondary material (SM) kg 1.92E+00 0 0 0 0 0
Use of renewable secondary fuels (RSF) MJ 0 0 0 0 0 0
Use of non renewable secondary fuels (NRSF) MJ 0 0 0 0 0 0
Use of net fresh water (FW) m3 2.61E+00 0 3.75E-05 0 4.79E-04 0
RESULTS OF THE LCA – WASTE CATEGORIES AND OUTPUT FLOWS according to EN 15804+A2:
1 m² ADAGIO HD+ mineral ceiling tiles (9.49 kg/m²)
Parameter Unit A1-A3 C1 C2 C3 C4 D
Hazardous waste disposed (HWD) kg 1.64E-05 0 1.46E-12 0 4.14E-11 0
Non hazardous waste disposed (NHWD) kg 3.26E+00 0 7.2E-05 0 9.5E+00 0
Radioactive waste disposed (RWD) kg 3.64E-03 0 8.85E-07 0 2.16E-05 0
Components for re-use (CRU) kg 0 0 0 0 0 0
Materials for recycling (MFR) kg 0 0 0 0 0 0
Materials for energy recovery (MER) kg 0 0 0 0 0 0
Exported electrical energy (EEE) MJ 0 0 0 0 0 0
Exported thermal energy (EET) MJ 0 0 0 0 0 0
RESULTS OF THE LCA – additional impact categories according to EN 15804+A2-optional:
1 m² ADAGIO HD+ mineral ceiling tiles (9.49 kg/m²)
Parameter Unit A1-A3 C1 C2 C3 C4 D
5 Environmental Product Declaration - Knauf Ceiling Solutions GmbH & Co. KG - ADAGIO HD+ (35 mm)
Disease
Incidence of disease due to PM emissions (PM) 4.27E-07 0 7.34E-10 0 1.24E-08 0
incidence
Human exposure efficiency relative to U235 (IR) kBq U235 eq 5.08E-01 0 1.32E-04 0 2.5E-03 0
Comparative toxic unit for ecosystems (ETP-fw) CTUe 2.99E+01 0 3.37E-01 0 1.03E+00 0
Comparative toxic unit for humans (carcinogenic) (HTP-c) CTUh 8.37E-09 0 6.84E-12 0 1.59E-10 0
Comparative toxic unit for humans (noncarcinogenic) (HTP-nc) CTUh 1.54E-07 0 3.05E-10 0 1.68E-08 0
Soil quality index (SQP) SQP 1.18E+02 0 1.97E-01 0 4.61E-01 0
Disclaimer 1 – for the indicator 'Potential Human exposure efficiency relative to U235'.
This impact category deals mainly with the eventual impact of low-dose ionizing radiation on human health of the nuclear fuel cycle. It
does not consider effects due to possible nuclear accidents, occupational exposure or radioactive waste disposal in underground
facilities. Potential ionizing radiation from the soil, radon and from some construction materials is also not measured by this indicator.
Disclaimer 2 – for the indicators 'abiotic depletion potential for non-fossil resources', 'abiotic depletion potential for fossil resources',
'water (user) deprivation potential, deprivation-weighted water consumption', 'potential comparative toxic unit for ecosystems', 'potential
comparative toxic unit for humans – cancerogenic', 'Potential comparative toxic unit for humans - not cancerogenic', 'potential soil
quality index'. The results of this environmental impact indicator shall be used with care as the uncertainties on these results are high
as there is limited experience with the indicator.
6. LCA: Interpretation
The following interpretation contains a summary of the LCA mineral ceiling tiles.
results referenced to a declared unit of 1 m² ADAGIO HD+
The comparison of the product's life cycle phases shows a C4) have a minor contribution.
clear dominance of the production phase (modules A1–A3) in
all environmental impact categories. The potential The upstream supply chain of the raw board plays a dominant
environmental impacts from transport to disposal (module C2) role in the carbon footprint.
and the End-of-Life of the products due to landfilling (module
7. Requisite evidence
7.1 Radioactivity 7.2 Biopersistence
Measurements of radioactivity did not reveal any evidence of The mineral wool used for the production of the panels is
artificial radioactivity outside the natural background radiation. biosoluble and, according to EU Regulation 1272/2008/EC, is
Measuring point: TÜV Süd Industrie Service to be assessed as free of suspected cancer. The "RAL Mineral
Wool Quality Seal" monitors and guarantees the quality of the
Test Number: G 7299 002 wool used.
Testing Date: 23.06.2021 The production and use of non-exempt fibres is prohibited by
6 Environmental Product Declaration - Knauf Ceiling Solutions GmbH & Co. KG - ADAGIO HD+ (35 mm)
the Ordinance on Hazardous Substances and the Chemicals
AgBB Overview (28 days)
Prohibition Ordinance.
Name Value Unit
7.3 VOC emissions TVOC (C6 - C16) 130 μg/m3
Measuring point: Eurofins Product Testing A/S Sum SVOC (C16 - C22) < 5 μg/m3
Test report: VOC emission test report Indoor Air Comfort GOLD
R (dimensionless) 0.11
(08.02.2021)
VOC without NIK < 5 μg/m3
Number: 392-2020-00524404_A_EN
Testing periode: 16.12.2020 - 13.01.2021 Carcinogenic substances < 1 μg/m3
Test basis: ISO 16000-6
8. References
Standards
DIN 18177 ISO 16000-6
DIN 18177:2012, Mineral tiles manufactured in the factory by ISO 16000-6:2011-12, Indoor air contaminants - Part 6:
the wet felt process - Characteristic values and test methods. Determination of VOCs in indoor air and test chambers,
sampling on Tenax TA®, thermal desorption and gas
EN 13501-1 chromatography with MS/FID.
DIN EN 13501-1:2019, Classification of construction products
and building elements according to their reaction to fire, Part 1: ISO 45001
Classification with the results of tests on the reaction to fire of DIN ISO 45001:2018-06, Occupational health and safety
construction products. management systems - Requirements with guidance for use.
EN 13964 ISO 50001
DIN EN 13964:2014, Suspended ceilings - Requirements and DIN EN ISO 50001:2011-12, Energy management systems -
test methods. Requirements with guidance for use.
EN 15804
DIN EN 15804:2012+A2:2019, Sustainability of construction Further References
works - Environmental product declarations - Core rules for the
product category of construction products. AgBB
Ausschuss zur gesundheitlichen Bewertung von Bauprodukte
ISO 354 (AgBB) (Committee for health-related evaluation of building
DIN EN ISO 354:2003-12, Acoustics - Measurement of sound products): Vorgehensweise bei der gesundheitlichen
absorption in reverberant rooms. Bewertung der Emissionen von flüchtigen organischen
Verbindungen (VOC und SVOC) aus Bauprodukten.
ISO 717-1
DIN EN ISO 717-1:2013-06, Acoustics - Assessment of sound AVV, German List of Wastes Ordinance
insulation in buildings and of building elements - Part 1: Regulation on the European Waste List.
Airborne sound insulation.
Chemicals Prohibition Ordinance
ISO 9001 Chemicals Prohibition Ordinance (German designation:
DIN EN ISO 9001:2015-11,Quality management systems - Chemikalien-Verbotsverordnung – ChemVerbotsV) of 20
Requirements. January 2017 (Federal Law Gazette I p. 94; 2018 I p. 1389),
last amended by Article 300 of the Ordinance of 19 June 2020
ISO 10848-2 (Federal Law Gazette I p. 1328).
DIN EN ISO 10848-2:2006-08, Acoustics - Measurement of
airborne and impact sound transmission between adjacent ECHA-candidate list
rooms in test stands - Part 2: Application to lightweight List of substances of very high concern (SVHC) for
components where the connection has a minor influence. authorisation (ECHA Candidate List), 25.06.2020, published
under Article 59(10) of REACH. Helsinki: European Chemicals
ISO 11654 Agency.
DIN EN ISO 11654:1997-07, Acoustics - Sound absorbers for
use in buildings - Evaluation of sound absorption. Eurofins Product Testing A/S
Test report: VOC emission test report Indoor Air Comfort GOLD
ISO 14001 (08.02.2021), Number: 392-2020-00524404_A_EN.
DIN EN ISO 14001:2015-11, Environmental management
systems - Requirements with guidance for use. IBU 2021
General instructions for the EPD program of Institut Bauen und
ISO 14025 Umwelt e.V. (IBU). Version 2.0, Berlin: Institut Bauen und
DIN EN ISO 14025:2011-10, Environmental labels and Umwelt e.V., 2021. www.ibu-epd.com
declarations — Type III environmental declarations —
Principles and procedures. LCA FE
LCA FE 10, LCA for Experts Software System and Database for
ISO 14044 Life Cycle Engineering. Version 10.7.1.28. Sphera, 1992-2023.
DIN EN ISO 14044:2006-10, Environmental management – Life
cycle assessment – Requirements and guidelines.
7 Environmental Product Declaration - Knauf Ceiling Solutions GmbH & Co. KG - ADAGIO HD+ (35 mm)
MLC 19.10.2023.
MLC 2023.2, Database for Life Cycle Engineering implemented
in LCA for Experts software system. DB v10.7 2023.2. Sphera, RAL Mineral Wool Quality Seal
1992-2023. Available at: GGM members with the right to use the RAL quality mark
https://sphera.com/productsustainabilitygabidatasearch/. including plants and fibre types, as of January 2021.
Ordinance on Biocide Products REACH
Regulation (EU) No 528/2012 of the European Parliament and Regulation (EC) No 1907/2006 of the European Parliament and
of the Council of 22 May 2012 concerning the making available Council from 18 December 2006, Regulation concerning the
on the market and use of biocidal products. Registration, Evaluation, Authorisation and Restriction of
Chemicals (REACH).
Ordinance on Hazardous Substances
Ordinance on Hazardous Substances, of 26 November 2010 Regulation (EU) Nr. 305/2011(CPR)
(Federal Law Gazette I p. 1643, 1644), last amended by Article Regulation (EU) No 305/2011 of the European Parliament and
148 of the Law of 29 March 2017 (Federal Law Gazette I p. of the Council of 9 March 2011 laying down harmonised
626). conditions for the marketing of construction products and
repealing Council Directive 89/106/EEC Text with EEA
PCR Part A relevance.
Product category rules for buildingrelated products and
services. Part A: Calculation rules for the life cycle assessment Regulation (EU) Nr.1272/2008
and requirements for the project report in accordance with EN Regulation (EC) No 1272/2008 of the European Parliament and
15804+A2:2019. Version 1.3. Berlin: Institut Bauen und Umwelt of the Council of 16 December 2008 on classification, labelling
e.V. (eds.), 2022. and packaging of substances and mixtures, amending and
repealing Directives 67/548/EEC and 1999/45/EC, and
PCR: Mineral panels amending Regulation (EC) No 1907/2006.
Institut Bauen und Umwelt e.V. (IBU), 2023. Product Category
Rules for Building-Related Products and Services. Part B: TÜV Süd Industrie Service
Requirements on the EPD for Mineral panels. Version 8. TÜV Strahlenmesslabor. IS-ETS1-MUC/er.
8 Environmental Product Declaration - Knauf Ceiling Solutions GmbH & Co. KG - ADAGIO HD+ (35 mm)
Publisher
Institut Bauen und Umwelt e.V. +49 (0)30 3087748- 0
Hegelplatz 1 info@ibu-epd.com
10117 Berlin www.ibu-epd.com
Germany
Programme holder
Institut Bauen und Umwelt e.V. +49 (0)30 3087748- 0
Hegelplatz 1 info@ibu-epd.com
10117 Berlin www.ibu-epd.com
Germany
Author of the Life Cycle Assessment
Daxner & Merl GmbH +43 676 849477826
Schleifmühlgasse 13/24 office@daxner-merl.com
1040 Wien www.daxner-merl.com
Austria
Owner of the Declaration
Knauf Ceiling Solutions GmbH & Co. KG 0049 8552 422 0
Elsenthal 15 ceiling.solutions@knauf.com
94481 Grafenau www.knaufceilingsolutions.com
Germany
9 Environmental Product Declaration - Knauf Ceiling Solutions GmbH & Co. KG - ADAGIO HD+ (35 mm)
