ENVIRONMENTAL PRODUCT DECLARATION
as per ISO 14025 and EN 15804+A2
Owner of the Declaration KONE Corporation
Publisher Institut Bauen und Umwelt e.V. (IBU)
Programme holder Institut Bauen und Umwelt e.V. (IBU)
Declaration number EPD-KON-20230581-CBA2-EN
Issue date 22.12.2023
Valid to 14.03.2028
Sliding Door 30 / 30E / 30T / 30ET / 30L / 30 LT / 60 / 60L
KONE
www.ibu-epd.com | https://epd-online.com
General Information
KONE Sliding Door 30 / 30E / 30T / 30ET / 30L / 30 LT / 60
/ 60L
Programme holder Owner of the declaration
IBU – Institut Bauen und Umwelt e.V. KONE Corporation
Hegelplatz 1 Keilasatama 3
10117 Berlin 02150 ESPOO
Germany Finland
Declaration number Declared product / declared unit
EPD-KON-20230581-CBA2-EN The declared unit is one piece (1 pc.) of the Sliding Door 30 without drive
comprising:
• Sliding panels,
• Side screens and
• Product packaging
This declaration is based on the product category rules: Scope:
Automatic doors, automatic gates, and revolving door systems, This EPD refers to the entire life cycle of a specific Sliding Door 30. The
01.08.2021 EPD is also representative for the Sliding Door 30E / 30T / 30 ET / 30L / 30
(PCR checked and approved by the SVR) LT / 60 / 60L. The production location is in Germany. Green electricity is
used at the production facility.
Issue date The year of data collection is 2022.
The owner of the declaration shall be liable for the underlying information
22.12.2023
and evidence; the IBU shall not be liable with respect to manufacturer
information, life cycle assessment data and evidences.
Valid to
The EPD was created according to the specifications of EN 15804+A2. In
14.03.2028 the following, the standard will be simplified as EN 15804.
Verification
The standard EN 15804 serves as the core PCR
Independent verification of the declaration and data according to ISO
14025:2011
internally X externally
Dipl.-Ing. Hans Peters
(Chairman of Institut Bauen und Umwelt e.V.)
Florian Pronold Dr.-Ing. Wolfram Trinius,
(Managing Director Institut Bauen und Umwelt e.V.) (Independent verifier)
1 Environmental Product Declaration - KONE - Sliding Door 30 / 30E / 30T / 30ET / 30L / 30 LT / 60 / 60L
Product
• High stability and torsional rigidity
Product description/Product definition • Low k-value of frame due to double glazing
The sliding door systems 30 and 60 comprise a sliding door • Excellent insulation features thanks to interlocking side
operator including sensors and control unit. The sliding doors seals and top and bottom seals
can be opened on one or two sides and configured with or • Flexible and adaptable to project requirements
without side screens.
Performance data of the product with respect to its
Thanks to the low profile width, the automatic sliding door characteristics in accordance with the relevant technical
systems 30 and 60 are extremely versatile and allow plenty of provision which can be applied are mentioned above.
light penetration. With various designs, the siliding doors are
the perfect solution for sophisticated projects. Base materials/Ancillary materials
To meet all requirements the systems can be combined with The major material composition including the packaging of the
different operator versions. For placing the sliding door systems product is listed below.
on the market the following legal provisions apply: Name Value Unit
• EN 16005 Glass 79 %
• DIN 18650-1/ -2 Aluminium 12 %
• ISO 13849-1
Plastics 7 %
• EN 60335-1
Steel 2 %
• EN 60335-2-103
• IEC 60335-2-103 The product contains partial articles which contain
• 2011/65/EU ROHS3 Directive substances listed in the Candidate List of REACH
Regulation 1907/2006/EC (date: 17.01.2023)
Application
exceeding 0.1 percentage by mass: no
The sliding door systems are an elegant solution for all
passage areas. The slender profile system provides visual The Candidate List can be found on the ECHA website
openness and stability in various configurations. On request, address: https://echa.europa.eu/de/home.
the automatic sliding door systems from KONE are
manufactured for individual dimensions of various building Reference service life
projects. Details regarding different operator systems that can The reference serivce life of the automatic sliding door systems
be combined with the profile systems are available in the amounts to 10 years, depending on the application and
respective product catalogues. frequency of use. For repairs and renewals, suitable spare
parts are available. The sliding doors are tested and certified to
Technical Data
EN 16005, meaning they are designed to withstand a minimum
• Low profile width of 1.000.000 cycles.
• Attractive glass surfaces thanks to slender frames
LCA: Calculation rules
The construction process stage includes:
Declared Unit — A4, transport to the building site;
The declared unit is 1 piece of the product: Automatic Sliding — A5, installation into the building;
Door 30 including provision of all materials, products and
Declared unit and mass reference energy, as well as waste processing up to the end-of
waste state or disposal of final residues during the
Name Value Unit
construction process stage.
Declared unit 1 pce.
Mass (total system) 252.73 kg
Use stage - Module B6
System boundary The use stage related to the operation of the building
The type of EPD is: cradle-to-gate with options, includes:
modules C1–C4, and module D (A1–A3 + C + D and — B6, operational energy use
additional modules: A4 + A5 + B6)
Production - Module A1-A3 End-of-life stage– Modules C1-C4 and D
The product stage includes: The end-of-life stage includes:
— A1, raw material extraction, processing and — C1, de-construction, demolition:
mechanical treatments, processing of secondary — C2, transport to waste processing;
material input (e.g. recycling processes), — C3, waste processing for reuse, recovery and/or
— A2, transport to the manufacturer, recycling;
— A3, manufacturing and assembly including provision — C4, disposal;
of all materials, products and energy, as well as waste including provision and all transport, provision of all
processing up to the end-of waste state. materials, products and related energy and water use.
Module D (Benefits and loads beyond the system
boundary) includes:
— D, recycling potentials, expressed as net impacts
Construction stage - Modules A4-A5 and benefits.
2 Environmental Product Declaration - KONE - Sliding Door 30 / 30E / 30T / 30ET / 30L / 30 LT / 60 / 60L
Geographic Representativeness Comparability
Land or region, in which the declared product system is Basically, a comparison or an evaluation of EPD data is only
manufactured, used or handled at the end of the product´s possible if all the data sets to be compared were created
lifespan: Global according to EN 15804 and the building context, respectively
the product-specific characteristics of performance, are taken
into account. Background database: GaBi, SP40.
LCA: Scenarios and additional technical information
Installation into the building (A5)
Characteristic product properties of biogenic carbon
Name Value Unit
Information on describing the biogenic Carbon Content at
Waste packaging (paper and plastic) 9 kg
factury gate
Name ValueUnit End of life (C1-C4)
Biogenic carbon content in accompanying kg C1: The product expansion depends on the building. The
0.003
packaging C product share is so low that no environmental burden is
assumed.
Note: 1 kg of biogenic carbon is equivalent to 44/12 kg of CO .
2
Name Value Unit
Collected separately waste type waste type 244 kg
The following technical scenario information is required for the Recycling 34.8 kg
declared modules.
Energy recovery 8.51 kg
Transport to the building site (A4) Landfilling 200 kg
Name Value Unit Transport to waste management 50 km
Litres of fuel (per 1 kg) 0.00276 l/100km
The product is disassembled in a recycling process. Material
Transport distance via medium truck 100 km recycling is then assumed for the metals, electronics and
Capacity utilisation (including empty runs) 55 % electromechanics. The plastic components are assumed to be
incinerated with energy recovery. Glass and minor proportions
Transport distance is declared for a distance of 100km by truck
of residues arising from the recycling process are landfilled.
in order to allow scaling to a specific point of installation.
Region for the End of Life is: Global.
3 Environmental Product Declaration - KONE - Sliding Door 30 / 30E / 30T / 30ET / 30L / 30 LT / 60 / 60L
LCA: Results
DESCRIPTION OF THE SYSTEM BOUNDARY (X = INCLUDED IN LCA; MND = MODULE OR INDICATOR NOT DECLARED; MNR
= MODULE NOT RELEVANT)
Benefits and
Construction loads beyond
Product stage Use stage End of life stage
process stage the system
boundaries
la ire ta m w a Ry lp p u s tro p s n a rT g n iru tc a fu n a M e h t m o rf tro p s n a rTe tis e h t o t e ta g y lb m e s s A e s U e c n a n e tn ia M ria p e R tn e m e c a lp e R tn e m h s ib ru fe R y g re n e la n o ita re p Oe s u re ta w la n o ita re p Oe s u n o itc u rts n o c -e Dn o itilo m e d tro p s n a rT g n is s e c o rp e ts a W la s o p s iD -e s u e R-y re v o c e R-g n ilc y c e Rla itn e to p
A1 A2 A3 A4 A5 B1 B2 B3 B4 B5 B6 B7 C1 C2 C3 C4 D
X X X X X MND MND MNR MNR MNR MND MND X X X X X
RESULTS OF THE LCA - ENVIRONMENTAL IMPACT according to EN 15804+A2: 1 piece Sliding Door 30 / 30E / 30T / 30ET /
30L / 30LT / 60 / 60L
Parameter Unit A1-A3 A4 A5 C1 C2 C3 C4 D
GWP-total kg CO 2 eq 4.54E+02 2.21E+00 2.29E+01 0 1.07E+00 2.17E+01 3.06E+00 -7.14E+01
GWP-fossil kg CO 2 eq 4.52E+02 2.11E+00 2.29E+01 0 1.02E+00 2.16E+01 3.04E+00 -7.12E+01
GWP-biogenic kg CO 2 eq 1.54E+00 9.8E-02 5.33E-04 0 4.7E-02 1.3E-02 1E-02 -1.2E-01
GWP-luluc kg CO 2 eq 1.91E-01 5.03E-05 1E-03 0 2.43E-05 1E-03 9E-03 -3.9E-02
ODP kg CFC11 eq 2.45E-10 2.23E-16 1.15E-14 0 1.08E-16 1.09E-14 1.13E-14 -3.04E-10
AP mol H+ eq 2.95E+00 2E-03 4E-03 0 1E-03 4E-03 2.2E-02 -2.21E-01
EP-freshwater kg P eq 4.16E-04 4.52E-07 1.84E-06 0 2.18E-07 1.74E-06 5.22E-06 -5.32E-05
EP-marine kg N eq 6.48E-01 6.73E-04 9.18E-04 0 3.24E-04 8.69E-04 6E-03 -3.4E-02
EP-terrestrial mol N eq 7.39E+00 7E-03 1.9E-02 0 4E-03 1.8E-02 6.2E-02 -3.68E-01
kg NMVOC
POCP 1.41E+00 2E-03 3E-03 0 9.17E-04 2E-03 1.7E-02 -1.05E-01
eq
ADPE kg Sb eq 7.62E-04 6.34E-08 1.58E-07 0 3.06E-08 1.5E-07 2.73E-07 -3.71E-04
ADPF MJ 6.73E+03 3E+01 1.06E+01 0 1.44E+01 1E+01 3.99E+01 -1.04E+03
m3 world eq
WDP 3.14E+01 4E-03 2.34E+00 0 2E-03 2.21E+00 3.19E-01 -7.95E+00
deprived
GWP = Global warming potential; ODP = Depletion potential of the stratospheric ozone layer; AP = Acidification potential of land and water; EP =
Eutrophication potential; POCP = Formation potential of tropospheric ozone photochemical oxidants; ADPE = Abiotic depletion potential for non-fossil
resources; ADPF = Abiotic depletion potential for fossil resources; WDP = Water (user) deprivation potential)
RESULTS OF THE LCA - INDICATORS TO DESCRIBE RESOURCE USE according to EN 15804+A2: 1 piece Sliding Door 30 /
30E / 30T / 30ET / 30L / 30LT / 60 / 60L
Parameter Unit A1-A3 A4 A5 C1 C2 C3 C4 D
PERE MJ 7.3E+02 9.4E-02 2.76E+00 0 4.6E-02 2.69E+00 5.22E+00 -3.53E+02
PERM MJ 8.4E-02 0 0 0 0 -8.4E-02 0 0
PERT MJ 7.3E+02 9.4E-02 2.76E+00 0 4.6E-02 2.61E+00 5.22E+00 -3.53E+02
PENRE MJ 6.07E+03 3E+01 3.98E+02 0 1.45E+01 2.85E+02 3.99E+01 -1.04E+03
PENRM MJ 6.62E+02 0 -3.87E+02 0 0 -2.75E+02 0 0
PENRT MJ 6.73E+03 3E+01 1.06E+01 0 1.45E+01 1E+01 3.99E+01 -1.04E+03
SM kg 2.59E+01 0 0 0 0 0 0 0
RSF MJ 0 0 0 0 0 0 0 0
NRSF MJ 0 0 0 0 0 0 0 0
FW m3 1.75E+00 1.7E-04 5.6E-02 0 8.17E-05 5.3E-02 1E-02 -6.98E-01
PERE = Use of renewable primary energy excluding renewable primary energy resources used as raw materials; PERM = Use of renewable primary
energy resources used as raw materials; PERT = Total use of renewable primary energy resources; PENRE = Use of non-renewable primary energy
excluding non-renewable primary energy resources used as raw materials; PENRM = Use of non-renewable primary energy resources used as raw
materials; PENRT = Total use of non-renewable primary energy resources; SM = Use of secondary material; RSF = Use of renewable secondary fuels;
NRSF = Use of non-renewable secondary fuels; FW = Use of net fresh water
RESULTS OF THE LCA – WASTE CATEGORIES AND OUTPUT FLOWS according to EN 15804+A2:
1 piece Sliding Door 30 / 30E / 30T / 30ET / 30L / 30LT / 60 / 60L
Parameter Unit A1-A3 A4 A5 C1 C2 C3 C4 D
HWD kg 1.04E-05 2.91E-09 4.04E-08 0 1.4E-09 3.82E-08 6.08E-07 -3.39E-06
NHWD kg 5.74E+01 3E-03 2.38E+00 0 1E-03 2.25E+00 2.01E+02 -1.1E+01
RWD kg 1.41E-01 3.22E-05 3.94E-04 0 1.55E-05 3.72E-04 4.54E-04 -8.6E-02
CRU kg 0 0 0 0 0 0 0 0
MFR kg 0 0 0 0 0 1.02E+01 0 0
MER kg 0 0 0 0 0 0 0 0
EEE MJ 0 0 4.24E+01 0 0 0 0 0
EET MJ 0 0 9.73E+01 0 0 0 0 0
4 Environmental Product Declaration - KONE - Sliding Door 30 / 30E / 30T / 30ET / 30L / 30 LT / 60 / 60L
HWD = Hazardous waste disposed; NHWD = Non-hazardous waste disposed; RWD = Radioactive waste disposed; CRU = Components for re-use;
MFR = Materials for recycling; MER = Materials for energy recovery; EEE = Exported electrical energy; EET = Exported thermal energy
RESULTS OF THE LCA – additional impact categories according to EN 15804+A2-optional:
1 piece Sliding Door 30 / 30E / 30T / 30ET / 30L / 30LT / 60 / 60L
Parameter Unit A1-A3 A4 A5 C1 C2 C3 C4 D
Disease
PM 1.93E-05 1.11E-08 5.2E-08 0 5.36E-09 4.92E-08 2.7E-07 -3.54E-06
incidence
IR kBq U235 eq 2.32E+01 5E-03 3.5E-02 0 2E-03 3.4E-02 4.7E-02 -1.63E+01
ETP-fw CTUe 7.48E+03 2.12E+01 3.98E+00 0 1.02E+01 3.77E+00 2.28E+01 -3.38E+02
HTP-c CTUh 3.34E-06 4E-10 3.45E-10 0 1.93E-10 3.26E-10 3.38E-09 -3.37E-08
HTP-nc CTUh 4.38E-06 1.71E-08 3.49E-08 0 8.24E-09 3.3E-08 3.72E-07 -4.67E-07
SQP SQP 3.89E+02 7.7E-02 3.18E+00 0 3.7E-02 3.01E+00 8.31E+00 -8.33E+01
PM = Potential incidence of disease due to PM emissions; IR = Potential Human exposure efficiency relative to U235; ETP-fw = Potential comparative
Toxic Unit for ecosystems; HTP-c = Potential comparative Toxic Unit for humans (cancerogenic); HTP-nc = Potential comparative Toxic Unit for humans
(not cancerogenic); SQP = Potential soil quality index
Disclaimer 1 – for the indicator “Potential Human exposure efficiency relative to U235”. This impact category deals mainly with the
eventual impact of low-dose ionizing radiation on human health of the nuclear fuel cycle. It does not consider effects due to possible
nuclear accidents, occupational exposure or radioactive waste disposal in underground facilities. Potential ionizing radiation from the
soil, radon and from some construction materials is also not measured by this indicator.
Disclaimer 2 – for the indicators “abiotic depletion potential for non-fossil resources”, “abiotic depletion potential for fossil resources”,
“water (user) deprivation potential, deprivation-weighted water consumption”, “potential comparative toxic unit for ecosystems”,
“potential comparative toxic unit for humans – cancerogenic”, “Potential comparative toxic unit for humans - not cancerogenic”,
“potential soil quality index”. The results of this environmental impact indicator shall be used with care as the uncertainties on these
results are high as there is limited experience with the indicator.
This EPD was created using a software tool.
References
DIN 18650-1
DIN 18650-1: 2010-06, ISO 14025
Powered pedestrian doors –Part 1: DIN EN ISO 14025:201110,
Product requirements and test methods. Environmental labels and declarations — Type III
environmental declarations — Principles and procedures.
DIN 18650-2
DIN 18650-2:2010-06, European Chemicals
Powered pedestrian doors –Part 2: Agency (ECHA)
Safety at powered pedestrian doors. https:echa.europa.eu/de/home
EN 15804 GaBi ts software
EN 15804:2012-04, Sustainability of construction works – Sphera Solutions GmbH
Environmental product declarations – Core rules for the product Gabi Software System and Database for Life Cycle
category of construction products; German version EN Engineering 1992-2020
15804:2012. Version 10.0.0.71
University of Stuttgart
EN 16005 Leinfelden-Echterdingen
EN 16005:2013-01, Power operated pedestrian doorsets -
Safety in use - Requirements and test methods; German GaBi ts documentation
version EN 16005:2012. GaBi life cycle inventory data documentation
(https://www.gabisoftware.com/support/gabi/gabidatabase-
EN 60335-1 2020-lci-documentation/).
EN 60335-1; VDE 0700-1:2012-10:2012-10,
Household and similar electrical appliances – Safety - IBU 2021
Part 1: General requirements (IEC 60335-1:2010, modified); General Instructions for the EPD programme of Institut Bauen
German version EN 60335-1:2012. und Umwelt e.V. Version 2.0, Berlin: Institut Bauen und Umwelt
e.V., 2021. www.ibu-epd.com.
EN 60335
EN 60335-2-103/A1; LCA-tool dormakaba
Household and similar electrical appliances - Safety - Part 2- LCA tool, ENS doors
103: Particularrequirements for drives for gates, doors and LCA tool no.: BU-DOR-202107-LT1-EN
windows (IEC 61/2863/CDV:2005); German version EN 60335- Developed by Sphera Solutions GmbH.
2-103:2003/prA1:2005.2011/65/EU.
PCR Part A
ISO 13849-1 PCR – Part A: Calculation Rules for the Life Cycle Assessment
ISO 13849-1:2008-12, and Requirements on the Project Re-port according to EN
Safety of machinery – Safetyrelated 15804+A2:2019, Version 1.0, Institut Bauen und Umwelt e.V.,
parts of control systems – Part 1: General www.ibu-epd.com.
principles for design (ISO 13849-1:2006.
5 Environmental Product Declaration - KONE - Sliding Door 30 / 30E / 30T / 30ET / 30L / 30 LT / 60 / 60L
PCR Part B Authorisation and Restriction of Chemicals.
PCR – Part B: Requirements on the EPD for Automatic doors,
automatic gates, and revolving door systems, 08.2021, Institut ROHS3 Directive
Bauen und Umwelt e.V., www.ibu-epd.com. Directive 2011/65/EU of the European Parliament and of the
Council of 8 June 2011 on the restriction of the use of certain
REACH Regulation hazardous substances in electrical and electronic equipment.
REACH Regulation (EC) No 1907/2006 of the European
Parliament and of the Council on the Registration, Evaluation,
6 Environmental Product Declaration - KONE - Sliding Door 30 / 30E / 30T / 30ET / 30L / 30 LT / 60 / 60L
Publisher
Institut Bauen und Umwelt e.V. +49 (0)30 3087748- 0
Hegelplatz 1 info@ibu-epd.com
10117 Berlin www.ibu-epd.com
Germany
Programme holder
Institut Bauen und Umwelt e.V. +49 (0)30 3087748- 0
Hegelplatz 1 info@ibu-epd.com
10117 Berlin www.ibu-epd.com
Germany
Author of the Life Cycle Assessment
dormakaba International Holding GmbH +49 2333 793-0
DORMA Platz 1 info.de@dormakaba.com
58256 Ennepetal www.dormakaba.com
Germany
Owner of the Declaration
KONE Corporation +358(0)204 75 1
Keilasatama 3 contact@kone.com
02150 ESPOO www.kone.com
Finland
7 Environmental Product Declaration - KONE - Sliding Door 30 / 30E / 30T / 30ET / 30L / 30 LT / 60 / 60L
