ENVIRONMENTAL PRODUCT DECLARATION
as per ISO 14025 and EN 15804+A2
Owner of the Declaration JACKON Insulation GmbH
Publisher Institut Bauen und Umwelt e.V. (IBU)
Programme holder Institut Bauen und Umwelt e.V. (IBU)
Declaration number EPD-JAC-20220371-CBA1-EN
Issue date 19/12/2023
Valid to 18/12/2028
JACKODUR EVO
Jackon Insulation GmbH
www.ibu-epd.com | https://epd-online.com
General Information
Jackon Insulation GmbH JACKODUR EVO
Programme holder Owner of the declaration
IBU – Institut Bauen und Umwelt e.V. JACKON Insulation GmbH
Hegelplatz 1 Carl-Benz-Straße 8
10117 Berlin 33803 Steinhagen
Germany Germany
Declaration number Declared product / declared unit
EPD-JAC-20220371-CBA1-EN The declared unit is 1 m3 of the XPS board, JACKODUR EVO.
This declaration is based on the product category rules: Scope:
Insulating materials made of foam plastics, 01/08/2021 JACKON Insulation, as data provider, produces the extruded polystyrene
(PCR checked and approved by the SVR) foam boards JACKODUR EVO containing CO as blowing agent and use
2
more than 5% post consumer recycled polystyrene (rGPPS) content plus
approximately 28% reclaimed/recovered content via internal recycling. The
Issue date data have been provided by one factory in Arendsee/Germany for the
19/12/2023 second half year 2022.
The owner of the declaration shall be liable for the underlying information
and evidence; the IBU shall not be liable with respect to manufacturer
information, life cycle assessment data and evidences.
Valid to
18/12/2028 The EPD was created according to the specifications of EN 15804+A2. In
the following, the standard will be simplified as EN 15804.
Verification
The standard EN 15804 serves as the core PCR
Independent verification of the declaration and data according to ISO
14025:2011
internally X externally
Dipl.-Ing. Hans Peters
(Chairman of Institut Bauen und Umwelt e.V.)
Florian Pronold Dr. Frank Werner,
(Managing Director Institut Bauen und Umwelt e.V.) (Independent verifier)
1 Environmental Product Declaration - Jackon Insulation GmbH - JACKODUR EVO
Product
Product description/Product definition Base materials/Ancillary materials
JACKODUR EVO is an extruded polystyrene foam (XPS) Name Value Unit
produced according to EN 13164 and available in board shape
GPPS 70 - 95 %
with a density range from 28 to 40 kg/m3, 34.37 kg/m3 in
rGPPS (post consumer) 5 - 30 %
average (measured). It has specifically low values of thermal
Blowing agents 6 - 8 %
conductivity. The boards can be delivered in various
compressive strength values from 300 to 700 kPa. To meet the Polymeric flame retardant 2 %
need of various applications the boards are produced with Additives 0.5 - 1 %
different surfaces: with the extrusion skin, planed, grooved or
JACKODUR EVO is made of polystyrene (90 to 95% by weight
with thermal embossing. JACKODUR EVO boards are supplied
– CAS 9003-53-6), blown with carbon dioxide (CAS 124-38-9)
with different edge treatments such as butt edge, ship-lap and
and halogen-free co-blowing agents altogether up to 8% by
tongue and groove. The EPD is related to an unlaminated
weight.
product only; lamination and additional product treatment
are not considered. For the placing on the market of the
product in the European Union/European Free Trade
For the production of JACKODUR EVO, internal production
Association (EU/EFTA) (with the exception of Switzerland)
scrap is recycled. According to the Italien "Piano d'Azione
Regulation (EU) No. 305/2011 (CPR) applies. The product
Nazionale sul GREEN PUBLIC PROCUREMENT (PANGPP)"
needs a declaration of performance taking into consideration
and the "Criteri ambientali minimi per l'affidamento del servizio
EN 13164 Building insulation and the CE-marking.
di progettazione ed esecuzione dei Lavori di Interventi edilizi"
the input of polystyrene is composed of:
Application
The variety of the performance properties of JACKODUR EVO
1. GPPS 40 - 70 %
make it suitable for use in a large number of applications such
2. rGPPS (internal scrap) 25 - 35%
as: perimeter insulation, inverted roof insulation, insulation of
3. rGPPS (post-consumer) 5 - 30%
pitched roofs, floor insulation including insulation of highly
loaded industrial floors, insulation of thermal bridges for exterior
The brominated polymeric flame retardant is used to enable the
walls, External Thermal Insulation Composite Systems
foam to meet fire performance standards. Other additives are
(ETICS), insulation of cavity walls, agricultural building ceiling
used, e.g. color pigments and processing aids in minor quantity.
insulation, prefabricated elements e.g. building sandwich
panels, insulation for building equipment and industrial
Polystyrene is produced from oil and gas. Therefore, it is linked
installations (pipe sections, ...)
to the availability of these raw materials. Polystyrene is
Technical Data transported by road.
Acoustic properties are not relevant for JACKODUR EVO. For
This product contains substances listed in the candidate list of
fire performance, these products achieve the fire classification
substances of very high concern (REACH Regulation,
Euroclass E according to EN 13501-1.
date:109.06.2023) exceeding 0.1 percentage by mass: no
Constructional data
Name Value Unit This product contains other Carcinogenic, Mutagenic,
Gross density 28 - 40 kg/m3 Reptrotoxic (CMR) substances in categories 1A or 1B which are
not on the candidate list, exceeding 0.1 percentage by mass:
0.3 -
Compressive strength acc. to EN 826 N/mm2 no
0.7
0.1 -
Tensile strength acc. to EN 1607 N/mm2 Biocide products were added to this construction product or it
0.4
has been treated with biocide products (this then concerns a
Calculation value for thermal conductivity 0.032 W/(mK) treated product as defined by the (EU) Ordinance on Biocide
Water vapour diffusion resistance factor acc. 50 - Products No. 528/2012): no
-
to EN 12088 250
Reference service life
Performance data of the product in accordance with the
A reference service life (RSL) according to ISO 15686 cannot
declaration of performance with respect to its essential
be declared. The durability of JACKODUR EVO is normally at
characteristics according to EN 13164:2012+A1:2015 Thermal
least as long as the lifetime of the building in which it is used
Insulation products for buildings.
(more than 80 years).
LCA: Calculation rules
JACKODUR EVO is available in several densities and
Declared Unit thicknesses. For a product with a density or thickness
The declared unit is 1 m3 of the XPS board, JACKODUR EVO. different from the reference density of 34.37 kg/m3, the
Declared unit environmental impacts may be calculated using the
following equation:
Name Value Unit
Declared unit 1 m3
Gross density 34.37 kg/m3
2 Environmental Product Declaration - Jackon Insulation GmbH - JACKODUR EVO
electricity and thermal energy generation are declared in
I – adapted Life Cycle Impact Assessment LCIA module D (D/1, D/2, and D/3).
adap
indicator or LCI parameter Modules C1-C4 and D
I – LCIA indicator or LCI parameter for reference The end-of-life stage includes:
ref
density of 34.37 kg/m3 • Manual dismantling (C1)
ρ – adapted density • Transport to EoL (C2)
adap
• Waste processing & disposal (C) with three 100 %
ρ – reference density 34.37 kg/m3
ref scenarios (scenario 1: thermal treatment (C3/1);
d – adapted board thickness
adap scenario 2: recycling(C3/2); scenario 3: landfill (C4/3)).
d ref – thickness of reference board 100mm • The resulting potential benefits for thermal and electrical
energy from energy substitution from incineration
System boundary (packaging material in A5 and the product in C3/1) and
Type of EPD according to EN 15804: "cradle to gate from recycling (C3/2) material benefit for the recycled
with options, modules C1–C4, and module D". The following material are considered in modules D/1 and D/2,
modules are declared: A1–A3, C, D and additional modules: A4 respectively. This affects only the rate of primary
+ A5. materials (no secondary materials). The benefits in D/3
solely account for the avoided burdens calculated by the
Modules A1-A3 inversion of the electricity grid mix and thermal energy
The product stage includes: from natural gas during packaging treatment (A5). This
• Raw material supply (A1) comprises the production of is considered under European conditions.
virgin and recycled polystyrene granulate, blowing and
Geographic Representativeness
co-blowing agents as well as flame retardants.
Land or region, in which the declared product system is
• The transport to the manufacturer is considered in
manufactured, used or handled at the end of the product´s
module A2.
lifespan: Europe
• The manufacturing of the XPS board (A3) comprises the
provision of all materials, products and energy, as well
as waste processing up to the end-of-waste state,
Comparability
including packaging of the product and the internal
Basically, a comparison or an evaluation of EPD data is only
recycling process of the foam scrap.
possible if all the data sets to be compared were created
Modules A4-A5
according to EN 15804 and the building context, respectively
The construction process stage includes:
the product-specific characteristics of performance, are taken
• Transport to the construction site (A4) into account. Background database: Sphera LCA FE (GaBi ts),
• Treatment of packaging material (A5) with benefit for CUP 2023.1
potential avoided burdens due to energy substitution of
LCA: Scenarios and additional technical information
Installation into the building (A5)
Characteristic product properties of biogenic carbon
No biogenic carbon is declared in the product or packaging. Name ValueUnit
Polyethylene foil (waste packaging to incineration) 0.434 kg
Information on describing the biogenic carbon content at
factory gate XPS pallets (waste packaging to incineration) 0.212 kg
Name ValueUnit
kg End of life (C1-C4)
Biogenic carbon content in product -
C For the End of Life stage, three different scenarios are
Biogenic carbon content in accompanying kg considered. One scenario with 100% incineration (C3/1),
-
packaging C another with 100% recycling (C3/2) and one scenario with
100% landfill (C4/3) are calculated.
Note: 1 kg of biogenic carbon content is equivalent to 44/12 kg
of CO Name Value Unit
2
Collected separately waste type (XPS) 34.37 kg
Energy recovery (C3/1) 34.37 kg
The values below refer to the declared unit of 1 m3 JACKODUR Recycling (C3/2) 34.37 kg
EVO XPS product.
Landfilling (C4/3) 34.37 kg
Transport to the building site (A4)
Name Value Unit
Litres of fuel 0.42 l/100km
Transport distance 500 km
Capacity utilisation (including empty runs) 61 %
Gross density of products transported 35.016 kg/m3
3 Environmental Product Declaration - Jackon Insulation GmbH - JACKODUR EVO
LCA: Results
The following tables display the environmentally relevant results according to EN 15804 for 1 m3 XPS board.
The three EoL scenarios are declared in modules C3/1 + D/1 (Scenario 1) and C3/2 + D/2 (Scenario 2) and C4/3 + D/3 (Scenario 3),
where:
• C3/1 represents the thermal treatment of XPS-boards,
• C3/2 the recycling of XPS, and
• C4/3 the landfilling of XPS.
Modules D/1, D/2 and D/3 include benefits and loads beyond the system boundary for the incineration of packaging materials and the
burning of the product during EoL scenario 1, recycling of the product in scenario 2, and landfilling of the product in scenario 3
respectively.
Module D/3 includes only benefits and loads beyond the system boundary of the treatment of packaging materials. No benefits are
declared from landfilling the XPS product.
DESCRIPTION OF THE SYSTEM BOUNDARY (X = INCLUDED IN LCA; ND = MODULE OR INDICATOR NOT DECLARED; MNR =
MODULE NOT RELEVANT)
Benefits and
Construction loads beyond
Product stage Use stage End of life stage
process stage the system
boundaries
la ire ta m w a Ry lp p u s tro p s n a rT g n iru tc a fu n a M e h t m o rf tro p s n a rTe tis e h t o t e ta g y lb m e s s A e s U e c n a n e tn ia M ria p e R tn e m e c a lp e R tn e m h s ib ru fe R y g re n e la n o ita re p Oe s u re ta w la n o ita re p Oe s u n o itc u rts n o c -e Dn o itilo m e d tro p s n a rT g n is s e c o rp e ts a W la s o p s iD -e s u e R-y re v o c e R-g n ilc y c e Rla itn e to p
A1 A2 A3 A4 A5 B1 B2 B3 B4 B5 B6 B7 C1 C2 C3 C4 D
X X X X X MND MND MNR MNR MNR MND MND X X X X X
RESULTS OF THE LCA - ENVIRONMENTAL IMPACT according to EN 15804+A2:
Parameter Unit A1-A3 A4 A5 C1 C2 C3/1 C3/2 C4/3 D/1 D/2 D/3
GWP-total kg CO 2 eq 1.04E+02 1.27E+00 2.09E+00 0 1.25E-01 1.15E+02 4.4E+00 2.44E+00 -4.73E+01 -6.83E+01 -1.01E+00
GWP-fossil kg CO 2 eq 1.03E+02 1.26E+00 2.09E+00 0 1.23E-01 1.15E+02 4.35E+00 2.44E+00 -4.72E+01 -6.8E+01 -1E+00
GWP-
biogenic kg CO 2 eq 4.79E-01 1.31E-04 6.93E-05 0 1.29E-05 3.65E-03 4.72E-02 3.19E-03 -5.58E-02 -2.71E-01 -1.19E-03
GWP-luluc kg CO 2 eq 1.71E-02 1.16E-02 2.21E-06 0 1.14E-03 1.38E-04 4.68E-04 1.95E-03 -2.91E-03 -4.07E-03 -6.19E-05
kg CFC11
ODP 1.42E-10 1.63E-13 9.79E-14 0 1.6E-14 5.32E-12 7.94E-11 3.97E-12 -2.29E-10 -6.95E-11 -4.88E-12
eq
AP mol H+ eq 1.44E-01 1.61E-03 1.97E-04 0 1.58E-04 1.01E-02 9.19E-03 7.09E-03 -4.95E-02 -1.06E-01 -1.05E-03
EP-
kg P eq 1.13E-04 4.59E-06 2.33E-08 0 4.5E-07 1.27E-06 1.61E-05 4.55E-04 -2.45E-05 -8.05E-05 -5.21E-07
freshwater
EP-marine kg N eq 4.19E-02 5.46E-04 4.21E-05 0 5.36E-05 2.22E-03 2.2E-03 1.62E-03 -1.61E-02 -2.92E-02 -3.42E-04
EP-terrestrial mol N eq 4.58E-01 6.57E-03 9.31E-04 0 6.45E-04 4.75E-02 2.3E-02 1.78E-02 -1.73E-01 -3.16E-01 -3.68E-03
kg NMVOC
POCP 2.84E-01 1.39E-03 1.25E-04 0 1.36E-04 6.52E-03 5.87E-03 5.16E-03 -4.57E-02 -1.14E-01 -9.72E-04
eq
ADPE kg Sb eq 3.44E-05 8.26E-08 9.1E-10 0 8.11E-09 4.93E-08 6.67E-07 6.25E-08 -1.38E-06 -2.04E-06 -2.93E-08
ADPF MJ 2.79E+03 1.71E+01 2.44E-01 0 1.68E+00 1.3E+01 9.06E+01 3.53E+01 -9.03E+02 -2.25E+03 -1.92E+01
m3 world eq
WDP 4.97E+00 1.52E-02 1.85E-01 0 1.49E-03 9.39E+00 9.59E-01 -3.34E-02 -1.98E+00 -1.39E+01 -4.2E-02
deprived
GWP = Global warming potential; ODP = Depletion potential of the stratospheric ozone layer; AP = Acidification potential of land and water; EP =
Eutrophication potential; POCP = Formation potential of tropospheric ozone photochemical oxidants; ADPE = Abiotic depletion potential for non-fossil
resources; ADPF = Abiotic depletion potential for fossil resources; WDP = Water (user) deprivation potential)
RESULTS OF THE LCA - INDICATORS TO DESCRIBE RESOURCE USE according to EN 15804+A2:
Parameter Unit A1-A3 A4 A5 C1 C2 C3/1 C3/2 C4/3 D/1 D/2 D/3
PERE MJ 7.72E+01 1.24E+00 6.25E-02 0 1.22E-01 3.37E+00 5.41E+01 3.18E+00 -7.09E+01 -4.62E+01 -1.51E+00
PERM MJ 0 0 0 0 0 0 0 0 0 0 0
PERT MJ 7.72E+01 1.24E+00 6.25E-02 0 1.22E-01 3.37E+00 5.41E+01 3.18E+00 -7.09E+01 -4.62E+01 -1.51E+00
PENRE MJ 1.6E+03 1.72E+01 2.89E+01 0 1.68E+00 1.18E+03 9.06E+01 3.53E+01 -9.03E+02 -2.26E+03 -1.92E+01
PENRM MJ 1.19E+03 0 -2.86E+01 0 0 -1.17E+03 -1.17E+03 0 0 0 0
PENRT MJ 2.79E+03 1.72E+01 2.44E-01 0 1.68E+00 1.3E+01 -1.08E+03 3.53E+01 -9.03E+02 -2.26E+03 -1.92E+01
SM kg 2.39E+00 0 0 0 0 0 0 0 0 3.04E+01 0
RSF MJ 0 0 0 0 0 0 0 0 0 0 0
NRSF MJ 0 0 0 0 0 0 0 0 0 0 0
FW m3 4.37E-01 1.36E-03 4.32E-03 0 1.34E-04 2.2E-01 4.37E-02 3.48E-04 -1.18E-01 -3.46E-01 -2.52E-03
PERE = Use of renewable primary energy excluding renewable primary energy resources used as raw materials; PERM = Use of renewable primary
energy resources used as raw materials; PERT = Total use of renewable primary energy resources; PENRE = Use of non-renewable primary energy
excluding non-renewable primary energy resources used as raw materials; PENRM = Use of non-renewable primary energy resources used as raw
materials; PENRT = Total use of non-renewable primary energy resources; SM = Use of secondary material; RSF = Use of renewable secondary fuels;
NRSF = Use of non-renewable secondary fuels; FW = Use of net fresh water
4 Environmental Product Declaration - Jackon Insulation GmbH - JACKODUR EVO
RESULTS OF THE LCA – WASTE CATEGORIES AND OUTPUT FLOWS according to EN 15804+A2:
Parameter Unit A1-A3 A4 A5 C1 C2 C3/1 C3/2 C4/3 D/1 D/2 D/3
HWD kg 1.79E-07 5.31E-11 5.35E-12 0 5.21E-12 2.71E-10 -7.09E-09 2.97E-09 -9.9E-08 -1.09E-07 -2.1E-09
NHWD kg 9.03E-01 2.62E-03 9.57E-03 0 2.57E-04 6.62E-01 6.63E-02 3.42E+01 -2.18E-01 -5.5E-01 -4.64E-03
RWD kg 5.06E-02 3.21E-05 1.47E-05 0 3.15E-06 7.82E-04 1.44E-02 4.18E-04 -7.96E-02 -1.31E-02 -1.69E-03
CRU kg 0 0 0 0 0 0 0 0 0 0 0
MFR kg 0 0 0 0 0 0 3.44E+01 0 0 0 0
MER kg 0 0 0 0 0 0 0 0 0 0 0
EEE MJ 0 0 4.22E+00 0 0 2.08E+02 0 0 0 0 0
EET MJ 0 0 7.5E+00 0 0 3.71E+02 0 0 0 0 0
HWD = Hazardous waste disposed; NHWD = Non-hazardous waste disposed; RWD = Radioactive waste disposed; CRU = Components for re-use;
MFR = Materials for recycling; MER = Materials for energy recovery; EEE = Exported electrical energy; EET = Exported thermal energy
RESULTS OF THE LCA – additional impact categories according to EN 15804+A2-optional:
Parameter Unit A1-A3 A4 A5 C1 C2 C3/1 C3/2 C4/3 D/1 D/2 D/3
Disease
PM 1.11E-06 1.18E-08 1.16E-09 0 1.16E-09 5.87E-08 7.74E-08 6.87E-08 -4.42E-07 -7.2E-07 -9.41E-09
incidence
IR kBq U235 eq 4.41E+00 4.79E-03 2.36E-03 0 4.7E-04 1.26E-01 2.4E+00 6.18E-02 -1.19E+01 -2.1E+00 -2.54E-01
ETP-fw CTUe 1.48E+03 1.21E+01 1.14E-01 0 1.19E+00 6.34E+00 3.99E+01 3.36E+01 -1.5E+02 -1.3E+03 -3.19E+00
HTP-c CTUh 2.87E-08 2.48E-10 1.29E-11 0 2.44E-11 6.46E-10 1.33E-09 1.55E-09 -5.64E-09 -2.64E-08 -1.2E-10
HTP-nc CTUh 1.29E-06 1.32E-08 3.89E-10 0 1.3E-09 2E-08 3.28E-08 1.29E-07 -2.64E-07 -1.07E-06 -5.6E-09
SQP SQP 6.18E+01 7.14E+00 7.7E-02 0 7.01E-01 4.13E+00 3.55E+01 3.06E+00 -6.99E+01 -3.22E+01 -1.49E+00
PM = Potential incidence of disease due to PM emissions; IR = Potential Human exposure efficiency relative to U235; ETP-fw = Potential comparative
Toxic Unit for ecosystems; HTP-c = Potential comparative Toxic Unit for humans (cancerogenic); HTP-nc = Potential comparative Toxic Unit for humans
(not cancerogenic); SQP = Potential soil quality index
Disclaimer 1 – for the indicator “Potential Human exposure efficiency relative to U235”. This impact category deals mainly with the
eventual impact of low-dose ionizing radiation on human health of the nuclear fuel cycle. It does not consider effects due to possible
nuclear accidents, occupational exposure or radioactive waste disposal in underground facilities. Potential ionizing radiation from the
soil, radon and from some construction materials is also not measured by this indicator.
Disclaimer 2 – for the indicators “abiotic depletion potential for non-fossil resources”, “abiotic depletion potential for fossil resources”,
“water (user) deprivation potential, deprivation-weighted water consumption”, “potential comparative toxic unit for ecosystems”,
“potential comparative toxic unit for humans – cancerogenic”, “Potential comparative toxic unit for humans - not cancerogenic”,
“potential soil quality index”. The results of this environmental impact indicator shall be used with care as the uncertainties on these
results are high as there is limited experience with the indicator.
References
Literature References means of guarded hot plate and heat flow meter
methods - Products of high and medium thermal
EN 15804 resistance
EN 15804:2012+A2:2019+AC:2021, Sustainability of
construction works — Environmental Product Declarations — EN 13164
Core rules for the product category of construction products. EN 13164: 2012 + A1: 201, Thermal insulation
products for buildings – Factory-made extruded
ISO 14025 polystyrene foam (XPS) products – Specification
EN ISO 14025:2011, Environmental labels and declarations —
Type III environmental declarations — Principles and EN 13501-1
procedures. EN 13501-1 + A1: 2018, Fire classification of
construction products and building elements - Part 1:
Classification using data from reaction to fire tests
Further References
EN 1607
Biocide regulation 2013-05 Thermal insulating products for building
Ordinance on Biocide Products No. 528/2012 applications – Determination of tensile strength
perpendicular to face
CPR
Regulation (EU) No. 305/2011 of the European Parliament and EN 826
of the Council, harmonized conditions for the marketing of 2013-05: Thermal insulation products for building
construction products applications – Determination of compression behaviour
EN 12088 IBU PCR PART A
2013-06: Thermal insulation products for building Product category rules for building- related productsand
applications – Determination of long-term water services. Part A, PCR - Part A: Calculation Rules for theLife
absorption by diffusion Cycle Assessment and Requirements on the Project
Reportaccording to EN 15804+A2:2019, version 1.3, Institut
EN 12667 Bauenund Umwelt e.V., 2022
2001-05: Thermal performance of buildings materials www.ibu-epd.com
and products – Determination of thermal resistance by
5 Environmental Product Declaration - Jackon Insulation GmbH - JACKODUR EVO
IBU PCR Part B prediction procedures
PCR – Part B: Insulating materials made of foam plastics,
version 7.0, Institut Bauen und Umwelt e.V., 2023 PANGPP
www.ibu-epd.com Action plan for the environmental sustainability of consumption
in the Public Administration sector, National Action Plan on
IBU 2021 Green Public Procurement, MINIMUM ENVIRONMENTAL
Institut Bauen und Umwelt e.V.: General Instructions for the CRITERIA FOR THE AWARDING OF THE DESIGN AND
EPD programme of Institut Bauen und Umwelt e.V., Version EXECUTION OF BUILDING WORK SERVICES
2.0, Berlin: Institut Bauen und Umwelt e.V., 2021
www.ibu-epd.com REACH
Regulation (EC) No 1907/2006 concerning the
ISO 14025 Registration, Evaluation, Authorisation and Restriction
DIN EN ISO 14025:2011-10, of Chemicals
Environmentaldesignations and declarations – Type III
Environmental Declarations – Basic principles and Sphera LCA FE (GaBi ts)
procedures Life Cycle Assessment for Experts (LCA FE) CUP 2023.1,
Sphera Solutions GmbH, GaBi Software System and Database
ISO 15686 for Life Cycle Engineering CUP Version: 2023.1, University of
ISO 15686-2:2012-05, Buildings and constructed Stuttgart, Leinfelden Echterdingen
assets - Service life planning - Part 2: Service life
6 Environmental Product Declaration - Jackon Insulation GmbH - JACKODUR EVO
Publisher
Institut Bauen und Umwelt e.V. +49 (0)30 3087748- 0
Hegelplatz 1 info@ibu-epd.com
10117 Berlin www.ibu-epd.com
Germany
Programme holder
Institut Bauen und Umwelt e.V. +49 (0)30 3087748- 0
Hegelplatz 1 info@ibu-epd.com
10117 Berlin www.ibu-epd.com
Germany
Author of the Life Cycle Assessment
Sphera Solutions GmbH +49 711 341817-0
Hauptstraße 111- 113 info@sphera.com
70771 Leinfelden-Echterdingen www.sphera.com
Germany
Owner of the Declaration
JACKON Insulation GmbH +49 5204 9955-0
Carl-Benz-Straße 8 info@jackodur.com
33803 Steinhagen www.jackon-insulation.com
Germany
7 Environmental Product Declaration - Jackon Insulation GmbH - JACKODUR EVO
