Environmental Product
Declaration
as per ISO 14025 and EN 15804+A2
Owner of the declaration: Synwer GmbH
Publisher: Kiwa-Ecobility Experts
Programme operator: Kiwa-Ecobility Experts
Registration number: EPD-Synwer-232-EN
Issue date: 07.11.2022
Valid to: 06.11.2027
Synwer® – Syn J 230 Sd 2
Diffusible, airtight and moisture-variable vapor barrier for interior and loft conversions
conversions
1. General information
Synwer GmbH Synwer – Syn J 230 Sd 2
Programme operator Owner of the declaration
Kiwa-Ecobility Experts Synwer GmbH
Voltastr. 5 Gierlichsstraße 23
13355 Berlin 53840 Troisdorf
Germany Germany
Registration number Declared product / declared unit
EPD-Synwer-232-EN 1 m2 vapor barrier
This declaration is based on the Product Scope
Category Rules Syn J 230 Sd 2 is a diffusible, airtight, and mois-
PCR B - Plastic and rubber sheets for roof, wall, ture-variable vapor barrier for interior and loft
and floor waterproofing, 2021-12-28 (draft) conversions. It is produced and distributed by
Issue date Synwer GmbH, located in Troisdorf (Ger-
07.11.2022 many). The EPD refers to the specific product.
EPD type: Cradle to gate with modules C1-C4
Valid to and module D
07.11.2027 Kiwa-Ecobility Experts shall not be liable with
respect to manufacturer information, life cy-
cle assessment data and evidence.
Verification
The European standard EN 15804+A2:2019
serves as the core PCR.
Independent verification of the declaration
and data according to ISO 14025:2011-10
☐internal ☒external
Frank Huppertz
(Head of Kiwa-Ecobility Experts)
Prof. Dr. Frank Heimbecher Niels Jonkers - PLUK sustainability
(Chairman of the independent expert committee – (Third party verifier)
Kiwa-Ecobility Experts)
Page | 2 Synwer GmbH – Syn J 230 Sd 2
2. Product
2.1 Product description
Syn J 230 Sd 2 is a diffusible, airtight, and moisture-variable vapor barrier for interior and loft conver-
sions made of polypropylene (PP) fleece and PP film. The PP film is glued together with the PP fleece
with a PU adhesive.
2.2 Application
Vapor barriers are mainly installed indoor, and they can be applied in the entire building. The product
can be also applied for the over-rafter insulation. The main purpose of the product is protection of the
building against penetrating moisture.
2.3 Technical data
Essential characteristics Unit Performance
Length (EN 1848-2) m 50
Width (EN 1848-2) m 1.50 -3.00 (+1.0/-0.4%)
Mass per unit area (EN 1849-2) g/m² 230 (±10)
Resistance to water penetration (EN 1928 Method A) - Passed
Water vapour transmission (DIN EN ISO 12572) m Sd > 2
Reaction to fire (EN 13501-1) - Test Report open
Tensile strength MD (EN 12311-1) N/50mm 380/50 (±30/50)
Tensile strength CD (EN 12311-1) N/50mm 300/50 (±30/50)
Elongation MD (EN 12311-1) % 50 (±20)
Elongation CD (EN 12311-1) % 65 (±20)
Tear resistance MD (EN 12310-1) N 300 (±30)
Tear resistance CD (EN 12310-1) N 390 (±30)
Durability
Aging (EN 1296) - Passed
Akali (EN 13984) - Passed
Shear resistance of joints - No performance declared
Water tightness of seams (EN 12691) - No performance declared
Resistance to impact - No performance declared
Hazardous substances - No
Temperature Resistance °C -40/+100
2.4 Placing on the market/ Application rules
In the EU/EFTA (excluding Switzerland) the placing on the market is covered by Regulation (EU) No.
305/2011 of 9 March 2011. For the product use the respective national provisions shall apply. The
products are packed and transported as rolls. The products need a declaration in accordance with EN
13984:2013 (Flexible sheets for waterproofing) and the CE marking.
Page | 3 Synwer GmbH – Syn J 230 Sd 2
2.5 Base materials / Ancillary materials
Syn J 230 Sd 2 is made of PP fleece, PP film and PU adhesive.
Raw material Unit Value
Polypropylene (PP) fleece % 76
Polypropylene (PP) film % 19
Polyurethan (PU) adhesive % 5
There is no biogenic carbon in the products.
The product does not contain substances listed on the "Candidate list of substances of very high con-
cern for authorisation" which exceed the limits for registration with EChA.
2.6 Manufacturing
The manufacturing is located at Synwer GmbH, Gierlichsstraße 23, 53840 Troisdorf, Germany. The PP
fleece as well as the PP film are already supplied and delivered as a finished product. The fleece is
laminated to the film. Prior to the lamination, the PU glue is melted in extruders and subsequently
applied to the fleece via slot dies. Subsequently a logo is printed on the product, and it is cut in size. If
necessary self-adhesive tapes are applied to the side edges of the side of the webs. Finally, the rolls
are stacked on reusable pallets and in packed in foil.
The manufacturing process is shown in the following figure:
Figure 1: Process flow chart of the production of Syn Sd 2/ 100
2.7 Packaging
Vapor barriers for interior and loft conversions are wrapped on a cardboard winding tube. The rolls
are than packed in PE film and stacked on reusable pallets, which are also packed in PE plastic film. All
packaging materials are recyclable or even reusable (pallets).
2.8 Reference Service Life (RSL)
The RSL of the product is strongly dependant on the RSL of the roof/building. If the product is installed
properly a RSL of 30 years can be assumed (BNB Service Life of Building Components).
Page | 4 Synwer GmbH – Syn J 230 Sd 2
3. LCA: Calculation rules
3.1 Declared unit
In accordance with the PCR B 1 m2 vapor barrier is chosen as the declared unit.
Product Unit Value
Declared unit m2 vapor barrier 1
Unit weight g/m2 230
Conversion factor to 1 kg - 4.35
3.2 System boundary
The EPD is a complete life cycle with a functional unit. It considers all potential environmental impacts
of the product from the cradle to the end of life. Table under LCA:Results provides an overview of the
information modules or product life cycle phases considered in the LCA. The manufacturing phase in-
cludes the production or extraction and processing of raw materials, the transport to the respective
production plant and the production of the vapor barrier. All inputs (raw materials, precursors, energy,
and auxiliary materials) as well as the by-products and waste are considered for all life cycle phases.
Finally, only production-related energy consumption (excluding administration and social rooms) is
considered.
The year 2020 represents the time reference for raw materials and electricity consumption. Due to the
production location Germany is considered as the geographical reference area. However, environmen-
tal effects such as the greenhouse effect can occur with a strong spatial and temporal offset.
The following production steps are considered during the manufacturing phase:
• Extraction and processing of the raw materials (fleece (PP), film (PP), adhesive (PU))
• Transport to the production site
• Processing of the products (lamination, printing, cutting, rewinding, finishing)
• Packaging (including packaging material)
• End-of-life (including transport)
Secondary fuels are not included in the production process and are therefore not considered. The
waste materials and quantities produced are included in the respective modules.
3.3 Estimates and assumptions
All datasets chosen for the LCA refer to the EU as the geographic reference. Transport distances for all
raw materials used (raw materials, operating materials, packaging) could be recorded. A payload factor
of 50 percent was used for all truck transports (suppliers, disposal transports and internal transports),
which corresponds to a full delivery and empty return trip. A data set for a non-specific truck was used
for phase A2. For the end-of-life waste scenario 100% incineration has been assumed. The end-of-life
waste scenario per input material has been chosen and for each row material 100% incineration has
been modeled.
3.4 Cut-off criteria
All flows that contribute more than 1% on the total mass, energy or environmental impact are included
in the LCA. It can be assumed that the neglected processes would have contributed less than 5% to the
impact categories considered. All process specific data could be determined and modelled using data-
base references from Ecoinvent.
Page | 5 Synwer GmbH – Syn J 230 Sd 2
3.5 Period under review
All process-specific data was collected for the operating year 2020. The quantities of raw and auxiliary
materials as well as energy consumption have been recorded and averaged over the entire operating
year 2020.
3.6 Data quality
Overall, the quality of the data can be considered as good. In the operating data survey, all relevant
process-specific data could be collected. The data relating to the manufacturing, transports and pack-
aging of vapor barriers for interior and loft conversions for pitch roof and wall were determined by the
Synwer GmbH.
Secondary data were taken from the EcoInvent database, version 3.6 (2019). The database is regularly
updated and thus complies with the requirements of ISO 14044 (background data not older than 10
years). The background data meets the requirements of EN 15804. The quantities of raw materials,
consumables and suppliers used as well as the energy consumption have been recorded and averaged
over the entire year of operation (2020). The general rule has been applied that specific data from
specific production processes or average data derived from specific processes must be given priority
when calculating an EPD or Life Cycle Assessment. Data for processes that the manufacturer cannot
influence or choose, were backed up with generic data.
The selection of the best fitting data sets is based on research and the help of experts. The transport
distances for the waste treatments as well as the used environmental profiles for loads and benefits
are based on the data from the NIBE EPD online application R<THiNK.
3.7 Allocation
Allocations were avoided as far as possible. There are no coproducts or byproduct in the manufactur-
ing of vapor barriers for interior and loft conversions for pitch deck and walls. Based on energy
consumption measurements, the energy requirements of production were allocated to the individual
products. Recyclable production waste (PP and PE fleece) is collected and sold to the third party. The
production waste sent to incineration is modelled through the combustion process of the specific
material and the avoided conventional energy production is credited in module D.
3.8 Comparability
In principle, a comparison or assessment of the environmental impacts of different products is only
possible if they have been prepared in accordance with EN 15804. For the evaluation of the
comparability, the following aspects have to be considered in particular: PCR used , functional or
declared unit, geographical reference, definition of the system boundary, declared modules, data
selection (primary or secondary data, background database, data quality), scenarios used for use and
disposal phases, and the life cycle inventory (data collection, calculation methods, allocations, validity
period). PCRs and general program instructions of different EPDs programs may differ. A comparability
needs to be evaluated. For further guidance see EN 15804+A2 (5.3 Comparability of EPD for
construction products) and ISO 14025 (6.7.2 Requirements for comparability).
Page | 6 Synwer GmbH – Syn J 230 Sd 2
4. LCA: Scenarios and additional technical information
For C1 it has been assumed that the product can be uninstalled manually by using hand cutting tools.
The end-of-life waste scenario per input material has been chosen and for each raw material 100%
incineration has been modeled under the consideration of suitable loads and benefits.
Note: The transport distances of the waste are based on the standard waste scenarios of the NMD
Determination Method (SBK 2019): incineration 150 km/ recycling 50 km / landfill 100 km; vehicle:
truck, unspecific. For energy recovery, it is assumed that only fossil raw materials are substituted, con-
sidering the calorific values of the raw materials of the declared product and energy and thermal effi-
ciencies of 18% and 32%. According the EN 15804, loads are credited in A3 or C3 to C4 and benefits
are credited in module D.
5. LCA: Results
The following tables show the results of the impact assessment indicators, resource use, waste and
other output streams. The results presented here refer to the declared specific product.
Disclaimer on ADP-e, ADP-f, WDP, ETP-fw, HTP-c, HTP-nc, SQP: The results of these environmental
impact indicators must be used with caution, as the uncertainties in these results are high or as there
is limited experience with the indicator.
Disclaimer on IRP: This impact category mainly addresses the potential effect of low dose ionizing ra-
diation on human health in the nuclear fuel cycle. It does not consider effects due to possible nuclear
accidents and occupational exposures, nor does it consider radioactive waste disposal in underground
facilities. Potential ionizing radiation from soil, radon, and some building materials is also not measured
by this indicator.
Page | 7 Synwer GmbH – Syn J 230 Sd 2
Description of the system boundary
Construction process Benefits and loads beyond
Product stage Use stage End of life stage
stage the system boundaries
la ir e t a m w a Ry lp p u s t r o p s n a r T u n a M-g n ir u t c a f t r o p s n a r Tu n a m m o r-
f
o t r e r u t c a fe s u fo e c a lp n o it c u r ts n o
C
n o it a lla ts n -is s e c o r p e s U n ia M-e c n a n e t r ia p e R tn e m e c a lp e
R
r u fe R-n e m h s ib la n o it a r e p Oe s u y g r e n e la n o it a r e p Oe s u r e t a w e D- n o it c u r ts n o cn o itilo m e d
/
t r o p s n a r T e ts a Wg n is s e c o r p la s o p s iD e s u e R-y r e v o c e R- g n ilc y c e R- a itn e t o pl
A1 A2 A3 A4 A5 B1 B2 B3 B4 B5 B6 B7 C1 C2 C3 C4 D
X X X MND MND MND MND MND MND MND MND MND X X X X X
X=Module declared | MND=Module not declared
Results of the LCA – Environmental impact: 1 m2 Syn J 230 Sd 2
Parameter Unit A1 A2 A3 C1 C2 C3 C4 D
Core environmental impact indicators (EN 15804+A2)
ADP-mm kg Sb-eqv 7,58E-06 5,15E-07 1,31E-06 0,00E+00 1,18E-07 1,00E-07 0,00E+00 -7,38E-07
ADP-f MJ 1,97E+01 3,07E-01 3,21E+00 0,00E+00 7,02E-02 6,89E-02 0,00E+00 -5,92E+00
AP mol H+ eqv. 2,39E-03 1,18E-04 7,39E-04 0,00E+00 2,70E-05 1,01E-04 0,00E+00 -7,52E-04
EP-fw kg PO4 eqv. 1,61E-05 2,05E-07 2,62E-05 0,00E+00 4,70E-08 6,79E-08 0,00E+00 -3,60E-05
EP-m kg N eqv. 4,18E-04 4,16E-05 1,50E-04 0,00E+00 9,52E-06 5,00E-05 0,00E+00 -1,39E-04
EP-t mol N eqv. 4,37E-03 4,58E-04 1,79E-03 0,00E+00 1,05E-04 5,22E-04 0,00E+00 -2,04E-03
GWP-b kg CO2 eqv. -4,41E-03 9,39E-06 -1,76E-02 0,00E+00 2,15E-06 1,24E-05 0,00E+00 -1,94E-02
GWP-f kg CO2 eqv. 6,51E-01 2,03E-02 2,30E-01 0,00E+00 4,66E-03 5,89E-01 0,00E+00 -4,03E-01
GWP-luluc kg CO2 eqv. 3,12E-04 7,45E-06 3,25E-04 0,00E+00 1,71E-06 1,29E-06 0,00E+00 -2,88E-04
GWP-total kg CO2 eqv. 6,47E-01 2,04E-02 2,13E-01 0,00E+00 4,66E-03 5,89E-01 0,00E+00 -4,23E-01
ODP kg CFC 11 eqv. 1,55E-08 4,49E-09 8,00E-09 0,00E+00 1,03E-09 6,80E-10 0,00E+00 -3,28E-08
POCP kg NMVOC eqv. 1,87E-03 1,31E-04 4,31E-04 0,00E+00 3,00E-05 1,25E-04 0,00E+00 -4,40E-04
WDP m3 world eqv. 5,20E-01 1,10E-03 6,22E-02 0,00E+00 2,51E-04 2,34E-03 0,00E+00 -8,78E-03
Additional environmental impact indicators (EN 15804+A2)
ETP-fw CTUe 7,33E+00 2,74E-01 3,49E+00 0,00E+00 6,26E-02 2,14E-01 0,00E+00 -2,17E+00
HTP-c CTUh 1,82E-10 8,87E-12 6,74E-11 0,00E+00 2,03E-12 2,26E-11 0,00E+00 -4,95E-11
HTP-nc CTUh 5,83E-09 2,99E-10 2,33E-09 0,00E+00 6,85E-11 8,86E-10 0,00E+00 -1,78E-09
IRP kBq U235 eqv. 1,54E-02 1,29E-03 8,08E-03 0,00E+00 2,94E-04 9,92E-05 0,00E+00 -1,13E-02
PM disease incidence 2,29E-08 1,83E-09 6,18E-09 0,00E+00 4,19E-10 4,53E-10 0,00E+00 -2,65E-09
SQP - 1,43E+00 2,66E-01 2,91E+00 0,00E+00 6,09E-02 1,86E-02 0,00E+00 -6,11E-01
ADP-mm=Abiotic depletion potential for non-fossil resources | ADP-f=Abiotic depletion for fossil resources potential | AP=Acidification potential, Accumulated Exceedance | EP-fw=Eutrophication potential, fraction of nutrients reaching
freshwater end compartment | EP-m=Eutrophication potential, fraction of nutrients reaching marine end compartment| EP-T=Eutrophication potential, Accumulated Exceedance | GWP-b=Global Warming Potential biogenic | GWP-
f=Global Warming Potential fossil fuels | GWP-luluc=Global Warming Potential land use and land use change |GWP-total=Global Warming Potential total| ODP=Depletion potential of the stratospheric ozone layer |POCP=Formation
potential of tropospheric ozone | WDP=Water (user) deprivation potential, deprivation- weighted water consumption | ETP-fw=Potential Comparative Toxic Unit for ecosystems | HTP-c=Potential Toxic Unit for Humans toxicity, cancer |
HTP-nc=Potential Toxic Unit for humans, non-cancer | IRP=Potential Human exposure efficiency relative to U235, human health | PM=Potential incidence of disease due to Particulate Matter emissions | SQP=Potential soil quality index
Page | 8 Synwer GmbH – Syn J 230 Sd 2
Results of the LCA – Resource u and environmental information: 1 m2 Syn J 230 Sd 2
Parameter Unit A1 A2 A3 C1 C2 C3 C4 D
PERE MJ 5,41E-01 3,84E-03 5,91E-01 0,00E+00 8,79E-04 1,41E-03 0,00E+00 -4,05E-01
PERM MJ 0,00E+00 0,00E+00 7,96E-02 0,00E+00 0,00E+00 0,00E+00 0,00E+00 0,00E+00
PERT MJ 5,41E-01 3,84E-03 6,74E-01 0,00E+00 8,79E-04 1,41E-03 0,00E+00 -4,05E-01
PENRE MJ 1,36E+01 3,26E-01 3,06E+00 0,00E+00 7,46E-02 7,52E-02 0,00E+00 -6,45E+00
PENRM MJ 7,51E+00 0,00E+00 3,25E-01 0,00E+00 0,00E+00 0,00E+00 0,00E+00 0,00E+00
PENRT MJ 2,11E+01 3,26E-01 3,44E+00 0,00E+00 7,46E-02 7,52E-02 0,00E+00 -6,45E+00
SM Kg 0,00E+00 0,00E+00 0,00E+00 0,00E+00 0,00E+00 0,00E+00 0,00E+00 0,00E+00
RSF MJ 0,00E+00 0,00E+00 0,00E+00 0,00E+00 0,00E+00 0,00E+00 0,00E+00 0,00E+00
NRSF MJ 0,00E+00 0,00E+00 0,00E+00 0,00E+00 0,00E+00 0,00E+00 0,00E+00 0,00E+00
FW M3 9,80E-03 3,74E-05 2,29E-03 0,00E+00 8,55E-06 9,70E-05 0,00E+00 -1,39E-03
HWD Kg 3,20E-06 7,77E-07 1,20E-06 0,00E+00 1,78E-07 5,95E-07 0,00E+00 -4,39E-06
NHWD Kg 3,17E-02 1,95E-02 1,80E-02 0,00E+00 4,45E-03 5,97E-03 0,00E+00 -1,35E-02
RWD Kg 1,32E-05 2,01E-06 9,92E-06 0,00E+00 4,61E-07 1,33E-07 0,00E+00 -1,47E-05
CRU Kg 0,00E+00 0,00E+00 0,00E+00 0,00E+00 0,00E+00 0,00E+00 0,00E+00 0,00E+00
MFR Kg 0,00E+00 0,00E+00 1,57E-02 0,00E+00 0,00E+00 0,00E+00 0,00E+00 0,00E+00
MER Kg 0,00E+00 0,00E+00 0,00E+00 0,00E+00 0,00E+00 0,00E+00 0,00E+00 0,00E+00
EE MJ 0,00E+00 0,00E+00 1,98E-02 0,00E+00 0,00E+00 0,00E+00 0,00E+00 0,00E+00
PERE=Use of renewable primary energy excluding renewable primary energy resources used as raw materials | PERM=Use of renewable primary energy resources used as raw materials | PERT=Total use of renewable primary energy resources
| PENRE= Use of non-renewable primary energy excluding non-renewable primary energy resources used as raw materials | PENRM=Use of non-renewable primary energy resources used as raw materials | PENRT=Total use of non-renewable
primary energy resources | SM=Use of secondary material | RSF=Use of renewable secondary fuels | NRSF=Use of non-renewable secondary fuels | FW=Use of fresh water | HWD=Hazardous waste disposed | NHWD=Non-hazardous waste
disposed | RWD=Radioactive waste disposed | CRU=Components for re-use | MFR=Materials for recycling | MER=Materials for energy recovery | EE=Exported energy
Page | 9 Synwer GmbH – Syn J 230 Sd 2
6. LCA: Interpretation
As shown in the figure below, A1 (raw material supply) and A3 (manufacturing) dominate in most
environmental core indicators. The highest impact among raw materiales is attributed to the fleece,
followed by the film. Lamination has the highest influence within the manufacturing phase (module
A3). The highest benefits beyond system boundaries (module D) orginate from the incineration of
virgin materials fleece and film at the end-of-life of the product. All transports (modules A2, C2) have
only a minor impact within all environmental core indicators.
100%
80%
60%
40%
20%
0%
-20%
-40%
-60%
ADP-mm ADP-f AP EP-fw EP-m EP-T GWP-total ODP POCP WDP
A1 A2 A3 C1 C2 C3 C4 D
Figure 2: Syn J 230 Sd 2 - Impact of the individual modules on the environmental core indicators
Page | 10 Synwer GmbH – Syn J 230 Sd 2
7. References
BNB Service Life of Building Components, https://www.nachhaltigesbauen.de/aus-
tausch/nutzungsdauern-von-bauteilen/, last assessed 2022-07-01
CML-IA April 2013 – Charakterisierungsfaktoren entwickelt durch Institut of Environmental Sciences
(CML): Universität Leiden, Niederlande - http://www.cml.leiden.edu/software/data-cmlia.html
Donndorf, R., Kahle H., Müller, G., Philipp H-J., Taschow, H-J., Wolf, O. (1973): Werkstoffeinsatz und
Korrosionsschutz in der chemischen Industrie. VEB Deutscher Verlag für Grundstoffindustrie Leipzig.
European Commission Joint Research Centre Institute for Prospective Technological Studies (JCR
2014): End-of-waste criteria for waste plastic for conversion, Seville, 2014, doi:10.2791/13033
Klöpffer, W., Grahl B.: Ökobilanz (LCA) – Ein Leitfaden für die Ausbildung und Beruf, Wily-VCH Ver-lag,
Weinheim, 2007
Rosauer, V. (2010): Abschätzung der herstellungsbedingten Qualität und Lebensdauer von Asphalt-
deckschichten mit Hilfe der Risikoanalyse (Estimation of the production-related quality and service life
of asphalt wearing courses with the aid of risk analysis). Technischen Universität Darmstadt, 2010
Protocol EPD-online - 25011.16.03.015 - Protocol EPD online - NMD, version 1.2, November 2016, NIBE
Standards and laws
ISO 14040:2006, Environmental management - Life cycle assessment - Principles and framework
ISO 14044:2006, Environmental management - Life cycle assessment - Requirements and guide-lines
ISO 14025:2006: Environmental labels and declarations — Type III environmental declarations — Prin-
ciples and procedures EN 13249
EN 15804:2012+A2:2019 Sustainability of construction works — Environmental Product Declarations
— Core rules for the product category of construction products
PCR A: General Program Category Rules for Construction Products from the EPD program Kiwa-Ecobil-
ity Experts, R.0_2021-07-16
PCR B: Product Category Rules (PCR) from the Kiwa-Ecobility Experts EPD program: “Product Category
Rules for plastic and rubber sheets for roof, wall, and floor waterproofing”, edition 2021-12-28 (draft)
Page | 11 Synwer GmbH – Syn J 230 Sd 2
Publisher E-mail DE.Ecobility.Ex-
Kiwa-Ecobility Experts perts@kiwa.com
Voltastr. 5 Web https://www.kiwa.com/de/
13355 Berlin de/themes/ecobility-ex-
Germany perts/ecobility-experts/
Programme operator E-mail DE.Ecobility.Ex-
Kiwa-Ecobility Experts perts@kiwa.com
Voltastr. 5 Web https://www.kiwa.com/de/
13355 Berlin de/themes/ecobility-ex-
Germany perts/ecobility-experts/
Author of the Life Cycle Tel. +49 (0)30 467761-43
Assessment Fax. +49 (0)30 467761-10
Kiwa GmbH E-mail DE.Nachhaltig-
Voltastr. 5 keit@kiwa.com
13355 Berlin Web https://www.kiwa.com/
Germany
Owner of the declaration Tel. +49(0) 2241 39 79 90-0
Synwer GmbH Fax. +49(0) 2241 39 79 9090
Gierlichsstraße 23 E-mail info@synwer.com
53840 Troisdorf
Germany Web https://www.synwer.com
Page | 12 Synwer GmbH – Syn J 230 Sd 2
