ENVIRONMENTAL PRODUCT DECLARATION
as per ISO 14025 and EN 15804+A2
Owner of the Declaration Knauf Ceiling Solutions GmbH & Co. KG
Programme holder Institut Bauen und Umwelt e.V. (IBU)
Publisher Institut Bauen und Umwelt e.V. (IBU)
Declaration number EPD­KNA­20210253­IBD1­EN
Issue date 05.11.2021
Valid to 04.11.2026
Knauf Ceiling Solutions Suspension System & Accessories
Knauf Ceiling Solutions GmbH & Co. KG
www.ibu-epd.com | https://epd-online.com
Umwelt Produktdeklaration Name des Herstellers – Name des Produkts
1. General Information
Knauf Ceiling Solutions GmbH & Co. KG Knauf Ceiling Solutions Suspension
System & Accessories
Programme holder Owner of the declaration
IBU – Institut Bauen und Umwelt e.V. Knauf Ceiling Solutions GmbH & Co. KG
Panoramastr. 1 Elsenthal 15
10178 Berlin 94481 Grafenau
Germany Germany
Declaration number Declared product / declared unit
EPD­KNA­20210253­IBD1­EN 1 linear metre (lm) grids with an average weight of
0.266 kg/lm produced by Knauf Ceiling Solutions.
This declaration is based on the product Scope:
category rules: This document refers to 1 linear metre (lm) grids as a
Metal ceilings, 01.2019 group average with a declared weight of 0.266 kg/lm
(PCR checked and approved by the SVR) produced by Knauf Ceiling Solutions. The grids are
manufactured at the organisation’s production sites in:
Issue date ­ Dreux (France)
05.11.2021 ­ Valenciennes (France)
­ Grafenau (Germany)
Valid to
04.11.2026 The product spectrum offers a high variety and
flexibility including various heights, widths and module
lengths. The declared unit was calculated based on the
average weight of the products of each analysed site
and weighted according to the production quantity of
each site. The conversion of the average product to
other specifications than the declared reference is
proportional to the product’s weight.
The owner of the declaration shall be liable for the
underlying information and evidence; the IBU shall not
be liable with respect to manufacturer information, life
cycle assessment data and evidences.
The EPD was created according to the specifications
of EN 15804+A2. In the following, the standard will be
simplified as EN 15804.
Verification
The standard EN 15804 serves as the core PCR
Independent verification of the declaration and data
according to ISO 14025:2010
Dipl. Ing. Hans Peters internally x externally
(chairman of Institut Bauen und Umwelt e.V.)
Dr. Alexander Röder Matthias Schulz
(Managing Director Institut Bauen und Umwelt e.V.)) (Independent verifier)
2. Product
2.1 Product description/Product definition This EPD applies to the following products:
Industrially manufactured metal ceiling systems acc. to
EN13964 made of edged or rolled metal sheets as DONN DX24, DONN DX3­ 24, DONN DX15, DONN
comprehensive construction kits or individual DX24 KB, DONN DX35, DONN Espace, DONN DP
components. Bandraster, DONN Perimeters.
A suspended ceiling system usually consists of main
runners, long and short cross tees, perimeters and Prelude 24, Prelude 24 Sixty², Prelude 15, Prelude 35,
other accessories. Prelude 24 CR, System Z, Prelude 24 NT+, Prelude 24
System S+, Javelin 24, Q­line T24, Prelude
Bandraster, Prelude Perimeters.
2 Environmental Product Declaration Knauf Ceiling Solutions GmbH & Co. KG – Knauf Ceiling Solutions Suspension
System & Accessories
VENTATEC Performance T24, VENTATEC sheet metal profile is transformed into a special profile
Performance T24 HIGH, VENTATEC Performance T15 with a complex geometry by incrementally bending the
HIGH, VENTATEC Perimeters. flat profile through a series of contoured and profiled
rolls. The sheet metal is usually coil­fed, but can also
Meridian, Rapid’Fix, VIC, Concealed grid, Accessories. be from a blank. Coil­fed roll forming equipment
produces complex profiles whose cross­sections can
For the placing on the market of the product in the be consistently produced, allowing very tight
European Union/European Free Trade Association tolerances, high­quality finishes and parts with very
(EU/EFTA) (with the exception of Switzerland) long lengths.
Regulation (EU) No. 305/2011 (CPR) applies. The
product needs a declaration of performance taking into 2.7 Environment and health during
consideration EN 13964:2014, suspended ceiling manufacturing
requirements and test methods and the CE­marking. The manufacturer complies with the special German
For the application and use the respective national and European regulations:
provisions apply.  All three manufacturing plants Dreux,
Grafenau and Valenciennes are ISO 9001
2.2 Application
and ISO 14001 certified.
Grids and Perimeters are typically used as
 Any waste generated is recycled
substructure of suspended ceilings. Their primary
function is to hold the ceiling tiles under normal  Not subject to declaration according to
conditions of use and also for special requirements REACH.
e.g. fire resistance.
A suspended ceiling system usually consists of main
runners, long and short cross tees and perimeters.
2.8 Product processing/Installation
There are no recognised systemic hazards associated
2.3 Technical Data
with the installation of a suspended ceiling
Suspension Systems are regulated by EN 13964 and
substructure. The use of suitable tools (e.g. plate
have corresponding labelling and declaration of
shears or cut­off grinders) for cutting the profiles must
performance. The following data provide an overview
be ensured.
of results:
2.9 Packaging
Constructional data
The profiles are packed into cardboard boxes and
Name Value Unit
stacked on pallets. Cardboard, paper and wood can be
Durability class (EN 13964) up to Class D ­
recycled in the usual ways.
Performance data of the product in accordance with
2.10 Condition of use
the declaration of performance with respect to its
When handled properly, the mechanical and structural­
essential characteristics according to EN 13964:2014,
physical properties of the profiles remain intact
suspended ceiling requirements and test methods (not
throughout the entire service life.
part of CE­marking).
2.11 Environment and health during use
2.4 Delivery status
A release of volatile organic compounds (VOC) or
The EPD refers to grids and perimeters with a steel
other substances from the profiles is not expected.
thickness from 0.25 ­ 0.7 mm (nominal) and a variable
length up to 6 m.
2.12 Reference service life
The service life of the profiles is up to 50 years,
2.5 Base materials/Ancillary materials
depending on the area of use, exposure and state of
The grids are made out of galvanised sheet steel in
maintenance.
combination with a capping made out of coated sheet
Within the framework of the conditions of use, no
steel or aluminium.
ageing effects are to be expected.
This product/article/at least one partial article contains
substances listed in the candidate list (date:
2.13 Extraordinary effects
25.06.2020) exceeding 0.1 percentage by mass: no.
Fire
This product/article/at least one partial article contains
The declared products are classified in the fire reaction
other carcinogenic, mutagenic and reprotoxic (CMR)
class A1 or A2­s1, d0 according to EN 13501-1. This
substances in categories 1A or 1B which are not on
means that they are "non­combustible" according to
the candidate list, exceeding 0.1 percentage by mass:
the German building authority designation (and also
no.
many other European countries) with negligible smoke
development and no burning drip in the event of fire.
Biocide products were added to this construction
product or it has been treated with biocide products
Fire protection
(this then concerns a treated product as defined by the
Name Value
(EU) Ordinance on Biocide Products No. 528/2012):
Building material class A2 / A1
no.
Smoke gas development s1 / ­
Burning droplets d0 / ­
2.6 Manufacture
The grids and perimeters are produced using roll
forming machines. In the roll forming process, a flat
3 Environmental Product Declaration Knauf Ceiling Solutions GmbH & Co. KG – Knauf Ceiling Solutions Suspension
System & Accessories
Water 2.14 Re-use phase
In the case of prolonged contact with water, rust may If the profiles are removed properly, they can be
occur on the punch and cut edges of the galvanised reinstalled.
profiles. If condensation is possible, the use of Otherwise, all profiles can be recycled up to 100%.
corrosion­resistant profiles is recommended.
2.15 Disposal
Mechanical destruction The waste code number of production residues for
Mechanical destruction leads to deformation of the steel according to the AVV, German List of
product and might lead to damages of the zinc layer. Wastes Ordinance is 17 04 07.
2.16 Further information
Further information at www.knaufceilingsolutions.com
3. LCA: Calculation rules
3.1 Declared Unit Disassembly of the product is done either manually or
This EPD refers to a declared unit of 1 linear metre using smaller tools. Referring energy demand is
(lm) grids with an average weight of 0.266 kg/lm considered to be negligible.
produced by Knauf Ceiling Solutions. The grids consist
of bent steel and two clips per grid (1.6 g per clip). Module C2 | transport to disposal
The transport to the disposal of the material is
Declared unit estimated declaring a 50 km radius to the disposal. In
Name Value Unit reality, this scenario may vary depending on the actual
Declared unit 1 rm location of deconstruction and referring waste
Weight 0.266 kg/lm treatment.
This study evaluates the environmental impact of grids Module C3 | waste processing
manufactured by Knauf Ceiling Solutions as a group Product flows that reach Module D for recycling reach
average. the end­of­waste state in C3 and thus leave the
product system. Environmental impacts resulting from
Knauf grids are manufactured at the organisation’s the grinding and sorting of steel scrap are not included,
production sites in Dreux (France), Valenciennes as referring energy demand is considered to be
(France) and Grafenau (Germany). The slitted coils negligible.
processed at the three sites are sourced centrally from
the company’s site in Antwerp (Belgium), where the Module C4 | disposal
slitting of the steel coils takes place. Module C4 refers to the emissions from the disposal of
the losses from waste processing. The chosen
The product spectrum offers a high variety and scenario, therefore, includes the environmental
flexibility including various heights, widths and module burdens of landfilling of 5 % of the material.
lengths. The declared unit was calculated based on the
average weight of the products of each analysed site Module D | benefits and loads beyond the system
and weighted according to the production quantity of boundary
each site. Grids consist of various steel components. Module D declares the recycling of the recovered steel
As a result, the conversion of the average product to (95 % of the product). It includes the potential for
other specifications than the declared reference is substituting primary steel.
proportional to the product’s weight.
3.3 Estimates and assumptions
Assumptions and approximations are applied in case
3.2 System boundary of a lack of representative data. All assumptions and
The life cycle assessment of average grid suspension approximations are documented precisely and
systems and accessories includes a cradle­to­gate represent a best­guess representation of reality. In
analysis of the products’ potential environmental case of uncertainty, a conservative approach is
impacts with modules C1–C4 and module D (A1–A3, + chosen.
C + D). Subsequent life cycle phases are part of the
analysis: 3.4 Cut-off criteria
The LCA model covers all available input and output
Module A1–A3 | Production stage flows, which can be represented based on robust data.
The production stage includes the upstream burdens Data gaps are filled with conservative assumptions
of raw material supply, their transports and the from average data (when available) or with generic
processing at the manufacturing plants located in data and are documented accordingly. Only data with
Dreux (France), Valenciennes (France) and Grafenau a contribution lower than 1 % were cut off. Thus, no
(Germany). In addition, the slitting of the coils takes data were neglected, of which a substantial impact is
place in Antwerp (Belgium). Grids and perimeters are to be expected. All relevant data were collected
produced via roll forming and bending of slitted steel comprehensively. Cut­off material and energy flows
coils. Main raw material inputs therefore represent hot­ were chosen carefully based on their expected
dip galvanized steel coils. The production sites are quantitative contribution as well as potential
supplied with electricity from the national power grids. environmental impacts. Thus, it can be assumed that
In addition, the French sites use thermal energy from the sum of all neglected input flows does not account
natural gas. for more than 5 % of the total material, water and
Module C1 | deconstruction and demolition energy flows.
4 Environmental Product Declaration Knauf Ceiling Solutions GmbH & Co. KG – Knauf Ceiling Solutions Suspension
System & Accessories
3.8 Allocation
3.5 Background data Background data for the supply chain of the hot­dip
This study uses generic background data for the galvanized steel are published by worldsteel (GaBi­
evaluation of upstream environmental impacts from databases). Representing an average of the global
GaBi databases (GaBi 10; 2021.2). steel industry, worldsteel background datasets ensure
a good geographical and technological representation
3.6 Data quality of steel production. All worldsteel datasets are
Data collection is based on product­specific modelled according to the worldsteel LCA
questionnaires. It follows an iterative process clarifying methodology, applying the system expansion approach
questions via e­mail, telephone calls or in for the allocation of co­products from steel production.
personal/web meetings. Intensive discussions between As a result, these datasets are not fully compliant with
Knauf Ceiling Solutions and Daxner & Merl results in the requirements of the EN 15804, which emphasises
an accurate mapping of product­related material and the so­called partitioning approach applying a
energy flows. This leads to a high quality of foreground subdivision of environmental impacts according to their
data collected. Data collection relies on a consistent physical relationships. Due to a lack of global data
process according to ISO 14044. calculated based on the partitioning approach, the
worldsteel datasets refer to the closest representation
The weighted average was calculated based on the of steel production in this context. Additionally, the
average product of the three production sites Dreux, deviation of the results of the two allocation
Valenciennes and Grafenau. Due to the similar approaches is to be expected under 5% according to
material specification, its representativity is considered Sphera. Scrap input is regarded as burden­free.
to be good.
All information for the allocation of given material and
The technological, geographical and time­related energy flows is based on the controlling systems of the
representativeness of the database was kept in mind three production sites. Annual input quantities are only
when selecting background data. Whenever specific available for the overall production site. The calculation
data were missing, either generic datasets or of the product­related input quantity is based on annual
representative average data were used instead. The scrap rates. Energy and other auxiliaries are allocated
implemented GaBi background datasets refer to the based on the linear meters produced.
latest versions available (not more than ten years old)
and are carefully chosen. 3.9 Comparability
Basically, a comparison or an evaluation of EPD data
3.7 Period under review is only possible if all the data sets to be compared
Foreground data were collected for the 2019 were created according to EN 15804 and the building
production year, and the data are based on the context, respectively the product­specific
volumes produced on an annual basis. characteristics of performance, are taken into account.
The GaBi background database was used to calculate
the LCA (GaBi 10; 2021.2).
4. LCA: Scenarios and additional technical information
Characteristic product properties Reuse, recovery and/or recycling potentials (D),
Information on biogenic Carbon relevant scenario information
The declared products do not contain any biogenic Name Value Unit
carbon. Net flow of steel scrap 0.256 kg/lm
Information on describing the biogenic Carbon
Content at factory gate
Name Value Unit
Biogenic Carbon Content in
0.003 kg C
accompanying packaging (pallet)
Biogenic Carbon Content in
accompanying packaging 0.002 kg C
(cardboard)
End of life (C1-C4)
Name Value Unit
Collected separately (steel) 0.266 kg
Recycling 95% 0.253 kg
Landfilling 5% 0.013 kg
5 Environmental Product Declaration Knauf Ceiling Solutions GmbH & Co. KG – Knauf Ceiling Solutions Suspension
System & Accessories
5. LCA: Results
The following table contains the LCA results for a declared unit of 1 linear metre (lm) grids with an average weight
of 0.266 kg/lm produced by Knauf Ceiling Solutions.
Disclaimer:
EP­freshwater: This indicator has been calculated as “kg P eq” as required in the characterization model
(EUTREND model, Struijs et al., 2009b, as implemented in ReCiPe;
http://eplca.jrc.ec.europa.eu/LCDN/developerEF.xhtml).
DESCRIPTION OF THE SYSTEM BOUNDARY (X = INCLUDED IN LCA; ND = MODULE OR INDICATOR NOT
DECLARED; MNR = MODULE NOT RELEVANT)
BENEFITS AND
CONSTRUCTI LOADS
PRODUCT STAGE ON PROCESS USE STAGE END OF LIFE STAGE BEYOND THE
STAGE SYSTEM
BOUNDARIES
6 Environmental Product Declaration Knauf Ceiling Solutions GmbH & Co. KG – Knauf Ceiling Solutions Suspension
System & Accessories
lairetam
waR
ylppus tropsnarT
gnirutcafunaM
eht
morf
tropsnarT
etis
eht
ot
etag
ylbmessA esU
ecnanetniaM
riapeR
tnemecalpeR tnemhsibrufeR
ygrene
lanoitarepO esu
retaw
lanoitarepO esu
noitcurtsnoc­eD
noitilomed tropsnarT
gnissecorp
etsaW
lasopsiD ­esueR ­yrevoceR ­gnilcyceR laitnetop
A1 A2 A3 A4 A5 B1 B2 B3 B4 B5 B6 B7 C1 C2 C3 C4 D
X X X ND ND ND ND MNR MNR MNR ND ND X X X X X
RESULTS OF THE LCA - ENVIRONMENTAL IMPACT according to EN 15804+A2: 1 lm grids (0.266 kg/lm)
Core Indicator Unit A1-A3 C1 C2 C3 C4 D
Global warming potential ­ total [kg CO2­Eq.] 7.94E­1 0.00E+0 8.04E­4 0.00E+0 6.44E­4 ­4.36E­1
Global warming potential ­ fossil fuels [kg CO2­Eq.] 8.11E­1 0.00E+0 7.99E­4 0.00E+0 6.50E­4 ­4.35E­1
Global warming potential ­ biogenic [kg CO2­Eq.] ­1.73E­2 0.00E+0 ­9.47E­7 0.00E+0 ­6.65E­6 ­2.48E­4
GWP from land use and land use change [kg CO2­Eq.] 2.78E­4 0.00E+0 6.50E­6 0.00E+0 6.50E­7 ­9.52E­6
Depletion potential of the stratospheric ozone layer [kg CFC11­Eq.] 1.13E­13 0.00E+0 1.57E­19 0.00E+0 1.53E­18 ­1.04E­15
Acidification potential, accumulated exceedance [mol H+­Eq.] 2.82E­3 0.00E+0 2.64E­6 0.00E+0 2.07E­6 ­7.74E­4
Eutrophication, fraction of nutrients reaching freshwater
[kg P­Eq.] 6.56E­7 0.00E+0 2.36E­9 0.00E+0 4.94E­10 ­9.46E­8
end compartment
Eutrophication, fraction of nutrients reaching marine end
[kg N­Eq.] 6.45E­4 0.00E+0 1.21E­6 0.00E+0 5.14E­7 ­1.49E­4
compartment
Eutrophication, accumulated exceedance [mol N­Eq.] 6.79E­3 0.00E+0 1.35E­5 0.00E+0 5.63E­6 ­1.51E­3
Formation potential of tropospheric ozone photochemical
[kg NMVOC­Eq.] 2.08E­3 0.00E+0 2.38E­6 0.00E+0 1.62E­6 ­6.68E­4
oxidants
Abiotic depletion potential for non­fossil resources [kg Sb­Eq.] 3.45E­6 0.00E+0 7.05E­11 0.00E+0 4.48E­11 ­1.08E­6
Abiotic depletion potential for fossil resources [MJ] 9.23E+0 0.00E+0 1.06E­2 0.00E+0 9.46E­3 ­4.26E+0
Water (user) deprivation potential, deprivation­weighted [m³ world­Eq
1.47E+1 0.00E+0 7.38E­6 0.00E+0 ­7.70E­6 ­1.19E+0
water consumption (WDP) deprived]
RESULTS OF THE LCA - INDICATORS TO DESCRIBE RESOURCE USE according to EN 15804+A2: 1 lm
grids (0.266 kg/lm)
Indicator Unit A1-A3 C1 C2 C3 C4 D
Renewable primary energy as energy carrier [MJ] 5.96E­1 0.00E+0 6.10E­4 0.00E+0 6.83E­4 2.68E­1
Renewable primary energy resources as material utilization [MJ] 1.19E­3 0.00E+0 0.00E+0 0.00E+0 0.00E+0 0.00E+0
Total use of renewable primary energy resources [MJ] 5.97E­1 0.00E+0 6.10E­4 0.00E+0 6.83E­4 2.68E­1
Non­renewable primary energy as energy carrier [MJ] 9.23E+0 0.00E+0 1.06E­2 0.00E+0 9.46E­3 ­4.26E+0
Non­renewable primary energy as material utilization [MJ] 5.11E­3 0.00E+0 0.00E+0 0.00E+0 0.00E+0 0.00E+0
Total use of non­renewable primary energy resources [MJ] 9.24E+0 0.00E+0 1.06E­2 0.00E+0 9.46E­3 ­4.26E+0
Use of secondary material [kg] 1.28E­2 0.00E+0 0.00E+0 0.00E+0 0.00E+0 2.56E­1
Use of renewable secondary fuels [MJ] 0.00E+0 0.00E+0 0.00E+0 0.00E+0 0.00E+0 0.00E+0
Use of non­renewable secondary fuels [MJ] 0.00E+0 0.00E+0 0.00E+0 0.00E+0 0.00E+0 0.00E+0
Use of net fresh water [m³] 3.43E­1 0.00E+0 6.98E­7 0.00E+0 9.77E­8 ­2.77E­2
RESULTS OF THE LCA – WASTE CATEGORIES AND OUTPUT FLOWS according to EN 15804+A2:
1 lm grids (0.266 kg/lm)
Indicator Unit A1-A3 C1 C2 C3 C4 D
Hazardous waste disposed [kg] 6.56E­9 0.00E+0 5.60E­13 0.00E+0 1.68E­12 9.31E­10
Non­hazardous waste disposed [kg] 2.15E­2 0.00E+0 1.67E­6 0.00E+0 1.33E­2 5.43E­2
Radioactive waste disposed [kg] 4.00E­5 0.00E+0 1.93E­8 0.00E+0 1.08E­7 4.62E­7
Components for re­use [kg] 0.00E+0 0.00E+0 0.00E+0 0.00E+0 0.00E+0 0.00E+0
Materials for recycling [kg] 0.00E+0 0.00E+0 0.00E+0 2.53E­1 0.00E+0 0.00E+0
Materials for energy recovery [kg] 0.00E+0 0.00E+0 0.00E+0 0.00E+0 0.00E+0 0.00E+0
Exported electrical energy [MJ] 0.00E+0 0.00E+0 0.00E+0 0.00E+0 0.00E+0 0.00E+0
Exported thermal energy [MJ] 0.00E+0 0.00E+0 0.00E+0 0.00E+0 0.00E+0 0.00E+0
RESULTS OF THE LCA – additional impact categories according to EN 15804+A2-optional:
1 lm grids (0.266 kg/lm)
Indicator Unit A1-A3 C1 C2 C3 C4 D
Potential incidence of disease due to PM emissions [Disease
4.58E­8 0.00E+0 1.50E­11 0.00E+0 2.24E­11 ­1.47E­8
Incidence]
Potential Human exposure efficiency relative to U235 [kBq U235­
1.34E­2 0.00E+0 2.82E­6 0.00E+0 1.55E­5 8.03E­3
Eq.]
Potential comparative toxic unit for ecosystems [CTUe] 1.74E+0 0.00E+0 7.86E­3 0.00E+0 2.78E­3 ­2.75E­1
Potential comparative toxic unit for humans ­ cancerogenic [CTUh] 5.44E­10 0.00E+0 1.59E­13 0.00E+0 3.23E­13 ­2.36E­10
Potential comparative toxic unit for humans ­ not cancerogenic [CTUh] 1.11E­8 0.00E+0 9.34E­12 0.00E+0 3.25E­11 ­5.25E­9
Potential soil quality index [­] 3.70E+0 0.00E+0 3.64E­3 0.00E+0 6.96E­4 6.38E­2
Disclaimer 1 – for the indicator “potential Human exposure efficiency relative to U235“.
This impact category deals mainly with the eventual impact of low dose ionizing radiation on human health of the
nuclear fuel cycle. It does not consider effects due to possible nuclear accidents, occupational exposure nor
radioactive waste disposal in underground facilities. Potential ionizing radiation from the soil, radon and from
some construction materials is also not measured by this indicator.
Disclaimer 2 – for the indicators: “abiotic depletion potential for fossil resources”, “abiotic depletion potential for
non­fossil resources”, “water (user) deprivation potential”, “deprivation­weighted water consumption”, “potential
comparative toxic unit for ecosystems”, “potential comparative toxic unit for humans ­ cancer effects”, “potential
comparative toxic unit for humans – non­cancer effects”, “potential soil quality index”.
The results of this environmental impact indicator shall be used with care as the uncertainties on these results are
high or as there is limited experience with the indicator.
6. LCA: Interpretation
The following interpretation contains a summary of the metre (lm) grids.
LCA results referenced to a declared unit of 1 linear
The comparison of the products’ life cycle phases spot in all of the impact categories considered except
shows a clear dominance of the production phase for potential ozone depletion.
(modules A1­A3). Environmental potentials in module
D refer to the recycling potential of primary steel. The deviation of the site­specific results from the
declared weighted average arrives at max. ± 20%.
When it comes to the environmental impacts in the
production phase of the grids, the production of the The conversion of the LCA results to specific products
hot­dip galvanized steel coils represents the major hot­ shows a linear correlation with the product weight.
7. Requisite evidence
7.1 VOC emissions
Not applicable as relevant clause for suspended ceiling
substructure components according to EN 13964.
7 Environmental Product Declaration Knauf Ceiling Solutions GmbH & Co. KG – Knauf Ceiling Solutions Suspension
System & Accessories
8. References
Standards Further References
EN 13501-1 AVV, German List of Wastes Ordinance
DIN EN 13501­1:2019, Classification of construction Regulation on the European Waste List.
products and building elements according to their
reaction to fire, Part 1: Classification with the results of Candidate list
tests on the reaction to fire of construction products. List of substances of very high concern (SVHC) for
authorisation (ECHA Candidate List), 25.06.2020,
EN 13964 published under Article 59(10) of REACH. Helsinki:
EN 13964:2014, suspended ceiling requirements and European Chemicals Agency.
test methods.
GaBi
EN 15804 GaBi 10, 2021.2. Software­System and Database for
DIN EN 15804:2020­03, Sustainability of construction Life Cycle Engineering. Stuttgart, Echterdingen:
works ­ Environmental Product Declarations ­ Core Sphera, 1992­2021. Available at:
rules for the product category of construction products. http://documentation.gabi­software.com.
German version EN 15804:2012+A2:2019.
IBU 2021
ISO 9001 Institut Bauen und Umwelt e.V.: General Programme
DIN EN ISO 9001:2015­11, Quality management Instructions for the Preparation of EPDs at the Institut
systems ­ Requirements. Bauen und Umwelt e.V., Version 2.0 Institut Bauen
und Umwelt e.V., 2021.
ISO 14001 www.ibu­epd.com
DIN EN ISO 14001:2015­11, Environmental
management systems ­ Requirements with guidance Ordinance on Biocide Products
for use. Regulation (EU) No 528/2012 of the European
Parliament and of the Council of 22 May 2012
ISO 14025 concerning the making available on the market and
DIN EN ISO 14025:2011­10, Environmental labels and use of biocidal products.
declarations ­ Type III environmental declarations ­
Principles and procedures. PCR Part A
Institut Bauen und Umwelt e.V. (IBU), 2021. Product
ISO 14044 Category Rules for Building­Related Products and
DIN EN ISO 14044:2006­10, Environmental Services. Part A: Calculation Rules for the Life Cycle
management ­ Life cycle assessment ­ Requirements Assessment and Requirements on the Project Report
and guidelines. according to EN 15804+A2:2019. Version 1.1.1,
15.04.2021.
PCR: Metal ceilings
Institut Bauen und Umwelt e.V. (IBU), 2019. Product
Category Rules for Building­Related Products and
Services. Part B: Requirements on the EPD for Metal
ceilings. Version 1.7., 08.01.2019.
Regulation (EU) No 305/2011
Regulation (EU) No 305/2011 of the European
Parliament and of the Council of 9 March 2011 laying
down harmonised conditions for the marketing of
construction products and repealing Council Directive
89/106/EEC.
8 Environmental Product Declaration Knauf Ceiling Solutions GmbH & Co. KG – Knauf Ceiling Solutions Suspension
System & Accessories
Publisher
Institut Bauen und Umwelt e.V. Tel +49 (0)30 3087748­ 0
Panoramastr. 1 Fax +49 (0)30 3087748­ 29
10178 Berlin Mail info@ibu­epd.com
Germany Web www.ibu-epd.com
Programme holder
Institut Bauen und Umwelt e.V. Tel +49 (0)30 ­ 3087748­ 0
Panoramastr 1 Fax +49 (0)30 – 3087748 ­ 29
10178 Berlin Mail info@ibu­epd.com
Germany Web www.ibu-epd.com
Author of the Life Cycle
Assessment Tel +43 676 849477826
Daxner & Merl GmbH Fax +43 42652904
Lindengasse 39/8 Mail office@daxner­merl.com
1070 Wien Web www.daxner-merl.com
Austria
Owner of the Declaration
Knauf Ceiling Solutions GmbH & Tel 0049 8552 422 0
Co. KG Fax 0049 8552 422 30
Elsenthal 15 Mail info@knaufamf.com
94481 Grafenau Web
Germany https://www.knaufceilingsoluti
ons.com
