ENVIRONMENTAL PRODUCT DECLARATION
as per ISO 14025 and EN 15804+A2
Owner of the Declaration Knauf Ceiling Solutions GmbH & Co. KG
Publisher Institut Bauen und Umwelt e.V. (IBU)
Programme holder Institut Bauen und Umwelt e.V. (IBU)
Declaration number EPD-KNA-20230242-IBA1-EN
Issue date 15.08.2023
Valid to 14.08.2028
TOPIQ Prime Hygena – Board
Knauf Ceiling Solutions GmbH & Co. KG
www.ibu-epd.com | https://epd-online.com
1. General Information
Knauf Ceiling Solutions GmbH & Co. KG TOPIQ Prime Hygena – Board
Programme holder Owner of the declaration
IBU – Institut Bauen und Umwelt e.V. Knauf Ceiling Solutions GmbH & Co. KG
Hegelplatz 1 Elsenthal 15
10117 Berlin 94481 Grafenau
Germany Germany
Declaration number Declared product / declared unit
EPD-KNA-20230242-IBA1-EN 1 m² TOPIQ Prime Hygena – Board panels with a surface weight of 2.04
kg/m².
This declaration is based on the product category rules: Scope:
Mineral panels, 01.08.2021 This document refers to 1 m² TOPIQ Prime Hygena – Board panels with a
(PCR checked and approved by the SVR) surface weight of 2.04 kg/m², manufactured at the production facility in
Grafenau, Germany.
Issue date The owner of the declaration shall be liable for the underlying information
and evidence; the IBU shall not be liable with respect to manufacturer
15.08.2023
information, life cycle assessment data and evidences.
The EPD was created according to the specifications of EN 15804+A2. In
Valid to
the following, the standard will be simplified as EN 15804.
14.08.2028
Verification
The standard EN 15804 serves as the core PCR
Independent verification of the declaration and data according to ISO
14025:2011
internally X externally
Dipl.-Ing. Hans Peters
(Chairman of Institut Bauen und Umwelt e.V.)
Florian Pronold Matthias Schulz,
(Managing Director Institut Bauen und Umwelt e.V.) (Independent verifier)
1 Environmental Product Declaration - Knauf Ceiling Solutions GmbH & Co. KG - TOPIQ Prime Hygena – Board
2. Product
This product/article/at least one partial article contains
2.1 Product description/Product definition substances listed in the ECHA-candidate list (date: 25.06.2020)
The ceiling tiles consist of mineral wool (rock wool) and a exceeding 0.1 percentage by mass: No
phenolic binder. The soft mineral tiles meet the requirements of
EN 13964. This product/article/at least one partial article contains other
carcinogenic, mutagenic, reprotoxic (CMR) substances in
The TOPIQ Prime Hygena - Board soft mineral tiles are categories 1A or 1B which are not on the candidate list,
available in different formats. exceeding 0.1 percentage by mass: No
For the placing on the market of the product in the European Biocide products were added to this construction product or it
Union/European Free Trade Association (EU/EFTA) (with the has been treated with biocide products (this then concerns a
exception of Switzerland) Regulation (EU) No. 305/2011 (CPR) treated product as defined by the (EU) Ordinance on Biocide
applies. The product needs a declaration of performance taking Products No. 528/2012): No
into consideration EN 13964:2014, suspended ceiling
requirements and test methods and the CE-marking. For the 2.6 Manufacture
application and use the respective national provisions apply. The raw boards for the TOPIQ soft mineral tiles are sourced
from Knauf Insulation from the plant in Nová Baňa (Slovakia),
2.2 Application see International EPD System EPD 2022.
Soft mineral tiles are typically used as lay-in for suspended
ceiling constructions. They are primarily used as optical In the Grafenau plant, the panels are laminated with a glass
cladding, but also for sound absorption and sound insulation, fleece, cut to size and the edges are machined. The TOPIQ
for fire resistance and against fire spreading as well as for tiles are painted with dispersion paint.
hygiene requirements.
The Grafenau factory is certified according to ISO 9001, ISO
2.3 Technical Data
14001, ISO 45001 and ISO 50001.
Soft Mineral boards are regulated by EN 13964 and have
corresponding labelling and declaration of performance. The 2.7 Environment and health during manufacturing
following data provide an overview of results: The manufacturer complies with the special German and
Construction data (according to DIN 18177) European regulations for the production of mineral slabs:
Name Value Unit • The manufacturing plant is certified according to ISO
9001, ISO 14001, ISO 45001 and ISO 50001.
Thermal conductivity 0.035W/(mK)
• The production has a closed water cycle.
Sound absorption coefficient acc. ISO 354 and
0.95 % • Production generates virtually no waste, all resulting
ISO 11654
blanks, dust and rejects are reused.
Airborne sound reduction acc. ISO 10848 and
13 dB • Exclusive use of mineral fibres according to Regulation
EN 717-1
(EU) No.1272/2008 Note Q.
Gross density (of the raw board) 110 kg/m3 • Prohibition of the production and use of biopersistent
Formaldehyde emissions acc. EN 717-1 13 μg/m3 fibres (Ordinance on Hazardous Substances, Annexe II,
No. 5).
Additional technical data are not relevant for this product. • Prohibition of placing biopersistent fibres on the market
(Chemicals Prohibition Ordinance, No.23 of the Annexe
Performance data of the product in accordance with the to §1).
declaration of performance with respect to its essential • Not subject to declaration according to REACH.
characteristics according to EN 13964:2014, suspended ceiling
requirements and test methods (not part of CE-marking). 2.8 Product processing/Installation
There are no recognised systemic hazards associated with the
2.4 Delivery status
installation of ceiling tiles. It is recommended that materials are
The EPD refers to tiles with a thickness of 15 mm which can handled in a manner that minimises dust generation. Workers
have variable length and width dimensions. should wear appropriate personal protective equipment.
Equipment such as gloves, goggles and dust masks are
2.5 Base materials/Ancillary materials
recommended to minimise exposure to dust and prevent skin
Mineral tile composition: irritation.
Name Value Unit
2.9 Packaging
Basalt 44-48 %
The panels are packaged in cardboard boxes and sealed with
Dolomite - Limestone 12-16 % transparent polyethylene film. These packages lie on
Recovered metallurgical slags 24 % chemically untreated wooden pallets. The pallets are wrapped
Thermo set resin binder 2-4 % with polyethylene stretch film. Foil, paper and wood can be
recycled in the usual ways.
Additives < 1 %
Fleece 9 %
Glue application rate 3 %
Biocide 0.001 % 2.10 Condition of use
Finish 7 % When handled properly, the mechanical and structural-physical
properties of the soft mineral tile remain intact throughout its
The recycled content is at least 28 %.
entire service life.
2 Environmental Product Declaration - Knauf Ceiling Solutions GmbH & Co. KG - TOPIQ Prime Hygena – Board
2.11 Environment and health during use Water
When properly installed, no dust/particles are released during Prolonged contact with water, can lead to a loss of structure,
the use phase. For the substance groups formaldehyde, volatile and if the soluble components are discharged into the sewage
organic compounds (VOCs) and total volatile organic treatment plant, they are biodegradable, increasing the
compounds (TVOCs), the limits according to DIN 18177 are chemical oxygen demand (COD) and biological oxygen
complied with. demand (BOD).
2.12 Reference service life
Mechanical destruction
The service life of the soft mineral tiles is up to 50 years, The soft mineral tiles can be broken by hand and also damaged
depending on the area of use, exposure and state of superficially, which can result in minor dust formation.
maintenance. Within the framework of the conditions of use, no
ageing effects are to be expected apart from visual 2.14 Re-use phase
discolouration caused by air circulation. If the panels are removed properly, they can be reinstalled. In
case of minor damage, the slabs can be reused as cut-to-size
2.13 Extraordinary effects
tiles. Mineral tiles can be returned to the manufacturing process
Fire if they are of the correct type and have sufficient material
The declared products are classified in the fire reaction class quality; they can be recycled up to 100 %.
A1 according to EN 13501-1. This means that they are "non-
combustible" according to the German building authority 2.15 Disposal
designation (and also many other European countries). The waste code number of production residues for mineral tiles
Fire Reaction according to the AVV, German List of Wastes Ordinance is 10
11 03, the waste code number for construction site waste
Name Value
(offcuts) is 17 06 04. If the tiles are not recycled as described in
Building material class A1
2.14., they are disposed of in a landfill.
Smoke gas development -
2.16 Further information
Burning droplets -
Further information at www.knaufceilingsolutions.com
DoPs at https://downloads.knaufceilingsolutions.com
3. LCA: Calculation rules
smaller tools. Referring energy demand is considered to be
3.1 Declared Unit negligible.
This EPD refers to a declared unit of 1 m² TOPIQ Prime
Hygena – Board panels with a surface weight of 2.04 kg/m² and Modul C2 | Transport to disposal
a thickness of 15 mm. The transport to the disposal of the material is estimated
Declared unit declaring a 50 km radius to the landfill. In reality, this scenario
may vary depending on the actual location of deconstruction
Name Value Unit
and referring waste treatment.
Declared unit 1 m2
Grammage 2.04 kg/m2 Module C3 | Waste processing
Layer thickness 0.015 m The declared scenario assumes landfilling of the product. The
referring environmental impacts are accounted for in module
The panels are produced at the Knauf Ceiling Solutions
C4.
production site in Grafenau, Germany under the brand name
TOPIQ.
Module C4 | Disposal
Various types of panels are produced at the site. A
Module C4 refers to the emissions from the disposal of the
differentiation between the product groups was made based on
stone wool panels. The chosen scenario, therefore, includes
the recipe of the products.
the environmental burdens of landfilling of the product.
3.2 System boundary
Module D | Benefits and loads beyond the system
The life cycle assessment of TOPIQ panels includes a cradle-
boundary
to-gate analysis of the products' environmental impacts with
The declared scenario assumes landfilling of the product.
modules (A1–A3, +C, +D). Subsequent life cycle phases are
Referring environmental impacts are accounted for in module
part of the analysis:
C4. There are no benefits and loads in module D.
Module A1–A3 | Production stage 3.3 Estimates and assumptions
The production stage includes the upstream burdens of raw
Assumptions and approximations are applied in case of a lack
material supply, their transports and the manufacturing
of representative data. All assumptions and approximations are
processes of the panels at the plant of Knauf Ceiling Solutions
documented precisely and represent a best-guess
located in Grafenau (Germany). Stone wool panels are coated
representation of reality. In case of uncertainty, a conservative
on site. Main raw material inputs, therefore, refer to stone wool
approach is chosen.
panels, fleece and adhesive. The production site is supplied
with electricity from the German power grid and thermal energy 3.4 Cut-off criteria
from natural gas. Also, the packaging of the products is The LCA model covers all available input and output flows,
considered. which can be represented based on robust data. Data gaps are
filled with conservative assumptions from average data (when
Module C1 | Deconstruction and demolition available) or with generic data and are documented
Disassembly of the product is done either manually or using accordingly. Only data with a contribution lower than 1 % were
3 Environmental Product Declaration - Knauf Ceiling Solutions GmbH & Co. KG - TOPIQ Prime Hygena – Board
cut off. Thus, no data were neglected, of which a substantial reference year of 2012. Due to a lack of other, more actual data
impact is to be expected. All relevant data were collected and its minor influence on the results, this dataset was deemed
comprehensively. Cut-off material and energy flows were as a suitable approximation for this assessment.
chosen carefully based on their expected quantitative
contribution as well as potential environmental impacts. Thus, it 3.7 Period under review
can be assumed that the sum of all neglected input flows does Foreground data were collected in the 2022 production year,
not account for more than 5 % of the total material, water and and the data are based on the volumes produced on an annual
energy flows. basis.
3.5 Background data 3.8 Geographic Representativeness
This study uses generic background data for the evaluation of Land or region, in which the declared product system is
upstream environmental impacts from GaBi databases (GaBi manufactured, used or handled at the end of the product´s
10; 2022.2). lifespan: Germany
3.6 Data quality 3.9 Allocation
Data collection is based on product-specific questionnaires. It All information for the allocation of given material and energy
follows an iterative process of clarifying questions via e-mail, flows is based on the Enterprise Resource Planning (ERP)-
telephone calls or in personal/web meetings. Intensive systems of the production site. Product-specific application
discussions between Knauf Ceiling Solutions and Daxner & rates of finish, adhesive, biocide and glass fleece were
Merl result in an accurate mapping of product-related material provided by the manufacturer. Furthermore, product-specific
and energy flows. This leads to a high quality of foreground input rates for electric and thermal energy as well as the
data collected. Data collection relies on a consistent process material efficiency during production were provided by Knauf
according to ISO 14044. Ceiling Solutions.
3.10 Comparability
The technological, geographical and time-related
Basically, a comparison or an evaluation of EPD data is only
representativeness of the database was kept in mind when
possible if all the data sets to be compared were created
selecting background data. Whenever specific data were
according to EN 15804 and the building context, respectively
missing, either generic datasets or representative average data
the product-specific characteristics of performance, are taken
were used instead. The implemented GaBi background
into account. The GaBi background database was used to
datasets refer to the latest versions available (not more than
calculate the LCA (GaBi 10; 2022.2).
ten years old) and are carefully chosen. n-butyl acrylate
represents an exception to this rule tracing back to the
4. LCA: Scenarios and additional technical information
Characteristic product properties of biogenic carbon
The declared product does not contain any biogenic carbon.
Information on the description of the biogenic carbon Assembly (A5)
content at the factory gate The End-of-Life of the product packaging is not declared in
Name ValueUnit module A5.
kg Name Value Unit
Biogenic carbon content in product -
C Packaging (cardboard) 0.047 kg/m²
Biogenic carbon content in accompanying 0.08 kg Packaging (pallets) 0.127 kg/m²
packaging C
Packaging (polyethylene-film) 0.0142 kg/m²
The carbon stored in the packaging was taken into account as
"CO -neutral". Thus the storage effect of the carbon bound in
2
End-of-Life (C1–C4)
the packaging is not included in the calculation but is
considered as emitted immediately. Name Value Unit
Collected separately 2.04 kg
Landfilling 2.04 kg
4 Environmental Product Declaration - Knauf Ceiling Solutions GmbH & Co. KG - TOPIQ Prime Hygena – Board
5. LCA: Results
The following table contains the LCA results for a declared unit of 1 m² TOPIQ Prime Hygena – Board panels with a surface weight of
2.04 kg/m² and a thickness of 15 mm.
DESCRIPTION OF THE SYSTEM BOUNDARY (X = INCLUDED IN LCA; ND = MODULE OR INDICATOR NOT DECLARED; MNR =
MODULE NOT RELEVANT)
Benefits and
Construction loads beyond
Product stage Use stage End of life stage
process stage the system
boundaries
la ire ta m w a Ry lp p u s tro p s n a rT g n iru tc a fu n a M e h t m o rf tro p s n a rTe tis e h t o t e ta g y lb m e s s A e s U e c n a n e tn ia M ria p e R tn e m e c a lp e R tn e m h s ib ru fe R y g re n e la n o ita re p Oe s u re ta w la n o ita re p Oe s u n o itc u rts n o c -e Dn o itilo m e d tro p s n a rT g n is s e c o rp e ts a W la s o p s iD -e s u e R-y re v o c e R-g n ilc y c e Rla itn e to p
A1 A2 A3 A4 A5 B1 B2 B3 B4 B5 B6 B7 C1 C2 C3 C4 D
X X X MND MND MND MND MNR MNR MNR MND MND X X X X X
RESULTS OF THE LCA - ENVIRONMENTAL IMPACT according to EN 15804+A2: 1 m² TOPIQ Prime Hygena – Board panels
(2.04 kg/m²)
Parameter Unit A1-A3 C1 C2 C3 C4 D
Global Warming Potential total (GWP-total) kg CO 2 eq 3.19E+00 0 6.19E-03 0 2.96E-02 0
Global Warming Potential fossil fuels (GWP-fossil) kg CO 2 eq 3.47E+00 0 6.15E-03 0 3.05E-02 0
Global Warming Potential biogenic (GWP-biogenic) kg CO 2 eq -2.81E-01 0 0 0 -9.03E-04 0
Global Warming Potential luluc (GWP-luluc) kg CO 2 eq 1.52E-03 0 4.13E-05 0 5.63E-05 0
Depletion potential of the stratospheric ozone layer (ODP) kg CFC11 eq 9.98E-12 0 6.02E-16 0 7.16E-14 0
Acidification potential of land and water (AP) mol H+ eq 2.61E-02 0 2.05E-05 0 2.16E-04 0
Eutrophication potential aquatic freshwater (EP-freshwater) kg P eq 5.02E-06 0 2.19E-08 0 5.17E-08 0
Eutrophication potential aquatic marine (EP-marine) kg N eq 2.23E-03 0 9.37E-06 0 5.53E-05 0
Eutrophication potential terrestrial (EP-terrestrial) mol N eq 2.46E-02 0 1.05E-04 0 6.07E-04 0
Formation potential of tropospheric ozone photochemical oxidants kg NMVOC
7.62E-03 0 1.84E-05 0 1.68E-04 0
(POCP) eq
Abiotic depletion potential for non fossil resources (ADPE) kg Sb eq 5.73E-07 0 6.18E-10 0 3.12E-09 0
Abiotic depletion potential for fossil resources (ADPF) MJ 5.27E+01 0 8.05E-02 0 3.99E-01 0
m3 world eq
Water use (WDP) 1.74E-01 0 6.86E-05 0 3.34E-03 0
deprived
RESULTS OF THE LCA - INDICATORS TO DESCRIBE RESOURCE USE according to EN 15804+A2: 1 m² TOPIQ Prime Hygena
– Board panels (2.04 kg/m²)
Parameter Unit A1-A3 C1 C2 C3 C4 D
Renewable primary energy as energy carrier (PERE) MJ 5.09E+00 0 5.58E-03 0 5.99E-02 0
Renewable primary energy resources as material utilization
MJ 4.83E+00 0 0 0 0 0
(PERM)
Total use of renewable primary energy resources (PERT) MJ 9.92E+00 0 5.58E-03 0 5.99E-02 0
Non renewable primary energy as energy carrier (PENRE) MJ 5.05E+01 0 8.08E-02 0 4E-01 0
Non renewable primary energy as material utilization (PENRM) MJ 2.21E+00 0 0 0 0 0
Total use of non renewable primary energy resources (PENRT) MJ 5.27E+01 0 8.08E-02 0 4E-01 0
Use of secondary material (SM) kg 5.98E-01 0 0 0 0 0
Use of renewable secondary fuels (RSF) MJ 0 0 0 0 0 0
Use of non renewable secondary fuels (NRSF) MJ 0 0 0 0 0 0
Use of net fresh water (FW) m3 1.01E-02 0 6.45E-06 0 1.01E-04 0
RESULTS OF THE LCA – WASTE CATEGORIES AND OUTPUT FLOWS according to EN 15804+A2:
1 m² TOPIQ Prime Hygena – Board panels (2.04 kg/m²)
Parameter Unit A1-A3 C1 C2 C3 C4 D
Hazardous waste disposed (HWD) kg 9.42E-07 0 4.28E-13 0 2.05E-11 0
Non hazardous waste disposed (NHWD) kg 5.31E-01 0 1.32E-05 0 2.05E+00 0
Radioactive waste disposed (RWD) kg 2.28E-03 0 1.5E-07 0 4.44E-06 0
Components for re-use (CRU) kg 0 0 0 0 0 0
Materials for recycling (MFR) kg 0 0 0 0 0 0
Materials for energy recovery (MER) kg 0 0 0 0 0 0
Exported electrical energy (EEE) MJ 0 0 0 0 0 0
Exported thermal energy (EET) MJ 0 0 0 0 0 0
RESULTS OF THE LCA – additional impact categories according to EN 15804+A2-optional:
1 m² TOPIQ Prime Hygena – Board panels (2.04 kg/m²)
Parameter Unit A1-A3 C1 C2 C3 C4 D
Incidence of disease due to PM emissions (PM) Disease 2.27E-07 0 1.17E-10 0 2.66E-09 0
5 Environmental Product Declaration - Knauf Ceiling Solutions GmbH & Co. KG - TOPIQ Prime Hygena – Board
incidence
Human exposure efficiency relative to U235 (IR) kBq U235 eq 1.77E-01 0 2.27E-05 0 4.93E-04 0
Comparative toxic unit for ecosystems (ETP-fw) CTUe 1.51E+01 0 5.7E-02 0 2.24E-01 0
Comparative toxic unit for humans (carcinogenic) (HTP-c) CTUh 6.71E-10 0 1.18E-12 0 3.41E-11 0
Comparative toxic unit for humans (noncarcinogenic) (HTP-nc) CTUh 2.77E-08 0 7.21E-11 0 3.78E-09 0
Soil quality index (SQP) SQP 9.86E+01 0 3.41E-02 0 8.31E-02 0
Disclaimer 1 – for the indicator 'Potential Human exposure efficiency relative to U235'.
This impact category deals mainly with the eventual impact of low-dose ionizing radiation on human health of the nuclear fuel cycle. It
does not consider effects due to possible nuclear accidents, occupational exposure or radioactive waste disposal in underground
facilities. Potential ionizing radiation from the soil, radon and from some construction materials is also not measured by this indicator.
Disclaimer 2 – for the indicators 'abiotic depletion potential for non-fossil resources', 'abiotic depletion potential for fossil resources',
'water (user) deprivation potential, deprivation-weighted water consumption', 'potential comparative toxic unit for ecosystems', 'potential
comparative toxic unit for humans – cancerogenic', 'Potential comparative toxic unit for humans - not cancerogenic', 'potential soil
quality index'.
The results of this environmental impact indicator shall be used with care as the uncertainties on these results are high as there is
limited experience with the indicator.
6. LCA: Interpretation
The following interpretation contains a summary of the LCA
results referenced to a declared unit of 1 m² TOPIQ Prime
Hygena – Board panels.
The comparison of the product's life cycle phases shows a climate change (GWP), as well as depletion of fossil resources
clear dominance of the production phase (modules A1–A3) in (ADPF).
all environmental impact categories. The potential
environmental impacts from transport to disposal (module C2) The emissions of biogenic greenhouse gases (GWP-biogenic)
and the End-of-Life of the products due to landfilling (module originate from the packaging of the rock mineral wool raw
C4) have a minor contribution. boards that is included in the used EPD results as well as the
packaging of the TOPIQ panels. Greenhouse-gas emissions
The environmental effects in the production phase are mainly from land use change (GWP luluc) result apart from the
dominated by the supply chain of the purchased rock mineral upstream supply chain of rock mineral wool boards, from
wool boards in all categories considered. As the representation transport as well as packaging. When it comes to the
of the upstream footprint of the raw board is based on a eutrophication potential of freshwater (EP-freshwater), also
product-specific EPD, a high quality of the results is to be packaging has a dominant role. Abiotic depletion potential for
expected. Furthermore, the supply chain of purchased energy non-fossil resources (ADPE) is also influenced by the top coat
carriers, especially electricity, has an influence on the potential as well as the adhesive system.
6 Environmental Product Declaration - Knauf Ceiling Solutions GmbH & Co. KG - TOPIQ Prime Hygena – Board
7. Requisite evidence
Number: 392-2022-00122903_A_EN
7.1 Radioactivity Testing period: 15.09.2022-13.10.2022
Measurements of radioactivity did not reveal any evidence of Test basis: ISO 16000-6
artificial radioactivity outside the natural background radiation.
AgBB Overview (28 days)
Measuring point: TÜV Süd Industrie Service
Name Value Unit
Test Number: G 7141 002
Testing Date: 14.12.2016 TVOC (C6 - C16) < 5 μg/m3
7.2 Biopersistence Sum SVOC (C16 - C22) < 5 μg/m3
The mineral wool used for the production of the panels is R (dimensionless) 0.13 -
biosoluble and, according to EU Regulation 1272/2008/EC, is
VOC without NIK < 5 μg/m3
to be assessed as free of suspected cancer. The "RAL Mineral
Carcinogenic substances < 1 μg/m3
Wool Quality Seal" monitors and guarantees the quality of the
wool used.
AgBB Overview (3 days)
The production and use of non-exempt fibres is prohibited by
Name Value Unit
the Ordinance on Hazardous Substances and the Chemicals
Prohibition Ordinance. TVOC (C6 - C16) 25 μg/m³
Sum SVOC (C16 - C22) < 5 μg/m³
7.3 VOC emissions R (dimensionless) 0.43 -
Measuring point: Eurofins Product Testing A/S
VOC without NIK < 5 μg/m³
Test report: VOC emission test report Indoor Air Comfort GOLD
Carcinogenic Substances < 1 μg/m³
(10.11.2022)
8. References
Standards ISO 11654
DIN EN ISO 11654:1997-07, Acoustics - Sound absorbers for
DIN 18177 use in buildings - Evaluation of sound absorption.
DIN 18177:2020-12, Wet-felt factory-produced mineral panels.
ISO 14001
EN 13501-1 DIN EN ISO 14001:2015-11, Environmental management
DIN EN 13501-1:2019, Classification of construction products systems - Requirements with guidance for use.
and building elements according to their reaction to fire, Part 1:
Classification with the results of tests on the reaction to fire of ISO 14025
construction products. DIN EN ISO 14025:2011-10, Environmental labels and
declarations — Type III environmental
EN 13964 declarations — Principles and procedures.
DIN EN 13964:2014, Suspended ceilings - Requirements and
test methods. ISO 14044
DIN EN ISO 14044:2006-10, Environmental management – Life
EN 15804 cycle assessment – Requirements and guidelines.
DIN EN 15804:2012+A2:2019+AC:2021, Sustainability of
construction works - Environmental product declarations - Core ISO 16000-6
rules for the product category of construction products. ISO 16000-6:2011-12, Indoor air contaminants - Part 6:
Determination of VOCs in indoor air and test chambers,
EN 16487 sampling on Tenax TA®, thermal desorption and gas
DIN EN 16487:2015-02, Acoustics - Test specifications for chromatography with MS/FID.
suspended ceilings - Sound absorption.
ISO 45001
ISO 354 DIN ISO 45001:2018-06, Occupational health and safety
DIN EN ISO 354:2003-12, Acoustics - Measurement of sound management systems - Requirements withguidance for use.
absorption in reverberant rooms.
ISO 50001
ISO 717-1 DIN EN ISO 50001:2011-12, Energy management systems -
DIN EN ISO 717-1:2013-06, Acoustics - Assessment of sound Requirements with guidance for use.
insulation in buildings and of building elements - Part 1:
Airborne sound insulation. Further References
ISO 9001 AgBB
DIN EN ISO 9001:2015-11, Quality management systems - Ausschuss zur gesundheitlichen Bewertung von Bauprodukte
Requirements. (AgBB) (Committee for health-related evaluation of building
products): Vorgehensweise bei der gesundheitlichen
ISO 10848 Bewertung der Emissionen von flüchtigen organischen
DIN EN ISO 10848:2006-08, Acoustics - Measurement of Verbindungen (VOC und SVOC) aus Bauprodukten.
airborne and impact sound transmission between adjacent
rooms in test stands. AVV, German List of Wastes Ordinance
Regulation on the European Waste List.
7 Environmental Product Declaration - Knauf Ceiling Solutions GmbH & Co. KG - TOPIQ Prime Hygena – Board
Chemicals Prohibition Ordinance
Chemicals Prohibition Ordinance (Germandesignation: PCR Part A
Chemikalien-Verbotsverordnung – ChemVerbotsV) of 20 Product category rules for building-related products and
January 2017 (Federal LawGazette I p. 94; 2018 I p. 1389), last services. Part A: Calculation rules for the life cycle assessment
amended by Article 300 of the Ordinance of 19 June 2020 and requirements on the project report according to
(Federal Law Gazette I p. 1328). EN15804+A2:2019. Version 1.3, Berlin: Institut Bauen und
Umwelt e.V. (Hrsg.), 2022.
ECHA-candidate list
List of substances of very high concern (SVHC) for PCR: Mineral panels
authorisation (ECHA Candidate List), 25.06.2020, published Institut Bauen und Umwelt e.V. (IBU), 2023. Product Category
under Article 59(10) of REACH. Helsinki: European Chemicals Rules for Building-Related Products and Services. Part B:
Agency. Requirements on the EPD for Mineral panels. Version v2,
31.05.2023.
Eurofins Product Testing A/S
Test report: VOC emission test report Indoor Air Comfort GOLD RAL Mineral Wool Quality Seal
(10.11.2022), Number: 392-2022-00122903_A_EN. GGM members with the right to use the RAL quality mark
including plants and fibre types, as of January 2021.
GaBi
GaBi 10, Software-System and Database for Life Cycle REACH
Engineering. DB 2022.2. Sphera, 1992-2022. Available at: Regulation (EC) No 1907/2006 of the European Parliament and
https://sphera.com/product-sustainability-gabi-data-search/. Council from 18 December 2006, Regulation concerning the
Registration, Evaluation, Authorisation and Restriction of
IBU 2021 Chemicals (REACH).
Institut Bauen und Umwelt e.V.: General instructions for the
EPD programme of Institut Bauen und Umwelt e.V. (IBU). Regulation (EU) Nr. 305/2011(CPR)
Version 2.0, Berlin: Institut Bauen und Umwelt e.V., 2021. Regulation (EU) No 305/2011 of the European Parliament and
www.ibuepd.com of the Council of 9 March 2011 laying down harmonised
conditions for the marketing of construction products and
International EPD System EPD 2022 repealing Council Directive 89/106/EEC Text with EEA
Environmental poduct declaration in accordance with ISO relevance.
14025, ISO 21930 and EN 15804+A2: PTN, TP from Knauf
Insulation Sprl. EPD registration number: S-P-05553, 2022. Regulation (EU) Nr.1272/2008
Regulation (EC) No 1272/2008 of the European Parliament and
Ordinance on Biocide Products of the Council of 16 December 2008 on classification, labelling
Regulation (EU) No 528/2012 of the European Parliament and and packaging of substances and mixtures, amending and
of the Council of 22 May 2012 concerning the making available repealing Directives 67/548/EEC and 1999/45/EC, and
on the market and use of biocidal products. amending Regulation (EC) No 1907/2006.
Ordinance on Hazardous Substances TÜV Süd Industrie Service
Ordinance on Hazardous Substances, of 26 November 2010 TÜV Strahlenmesslabor. IS-ETS1-MUC/er.
(Federal Law Gazette I p. 1643, 1644), last amended by Article
148 of the Law of 29 March 2017 (Federal Law Gazette I p.
626).
8 Environmental Product Declaration - Knauf Ceiling Solutions GmbH & Co. KG - TOPIQ Prime Hygena – Board
Publisher
Institut Bauen und Umwelt e.V. +49 (0)30 3087748- 0
Hegelplatz 1 info@ibu-epd.com
10117 Berlin www.ibu-epd.com
Germany
Programme holder
Institut Bauen und Umwelt e.V. +49 (0)30 3087748- 0
Hegelplatz 1 info@ibu-epd.com
10117 Berlin www.ibu-epd.com
Germany
Author of the Life Cycle Assessment
Daxner & Merl GmbH +43 676 849477826
Lindengasse 39/8 office@daxner-merl.com
1070 Wien www.daxner-merl.com
Austria
Owner of the Declaration
Knauf Ceiling Solutions GmbH & Co. KG 0049 8552 422 0
Elsenthal 15 info@knaufamf.com
94481 Grafenau www.knaufceilingsolutions.com
Germany
9 Environmental Product Declaration - Knauf Ceiling Solutions GmbH & Co. KG - TOPIQ Prime Hygena – Board
