ENVIRONMENTAL PRODUCT DECLARATION
as per ISO 14025 and EN 15804+A2
Owner of the Declaration Kingspan Insulation B.V.
Publisher Institut Bauen und Umwelt e.V. (IBU)
Programme holder Institut Bauen und Umwelt e.V. (IBU)
Declaration number EPD-KSI-202300167-CBA1-EN
Issue date 11.07.2023
Valid to 10.07.2028
Kooltherm® K12 D
Kingspan Insulation B.V.
www.ibu-epd.com | https://epd-online.com
General Information
Kingspan Insulation B.V. Kooltherm® K12 D
Programme holder Owner of the declaration
IBU – Institut Bauen und Umwelt e.V. Kingspan Insulation B.V.
Hegelplatz 1 Lingewei 8
10117 Berlin 4004LL Tiel
Germany Netherlands
Declaration number Declared product / declared unit
EPD-KSI-202300167-CBA1-EN Kooltherm® K12 D Framing Board
1 m², 100 mm thickness, R = 4,75 m²·K/W
D
This declaration is based on the product category rules: Scope:
Insulating materials made of foam plastics, 01.08.2021 The insulation material Kooltherm®, is produced by Kingspan Insulation
(PCR checked and approved by the SVR) B.V. at the manufacturing facility in Tiel, the Netherlands. A composite foil
based facing is autohesively bonded to the insulation core during
manufacture.
Issue date
In order to enable the user of the EPD to calculate the LCA results for
11.07.2023
different thicknesses, the EPD contains the respective calculation rules.
The owner of the declaration shall be liable for the underlying information
and evidence; the IBU shall not be liable with respect to manufacturer
Valid to
information, life cycle assessment data and evidences.
10.07.2028
The EPD was created according to the specifications of EN 15804+A2. In
the following, the standard will be simplified as EN 15804.
Verification
The standard EN 15804 serves as the core PCR
Independent verification of the declaration and data according to ISO
14025:2011
internally X externally
Dipl.-Ing. Hans Peters
(Chairman of Institut Bauen und Umwelt e.V.)
Florian Pronold Vito D'Incognito,
(Managing Director Institut Bauen und Umwelt e.V.) (Independent verifier)
1 Environmental Product Declaration - Kingspan Insulation B.V. - Kooltherm® K12 D
Product
Performance data of the product in accordance with the
Product description/Product definition declaration of performance with respect to its essential
Kooltherm® K12 D is a rigid thermoset cellular insulation characteristics according to EN 13166:2012+A2:2016 - Thermal
material faced on both sides with a composite foil based facing. insulation products for buildings - Factory made phenolic foam
The product is available in variable thicknesses from 20 mm up (PF) products - Specification
to 200 mm. This EPD is based on a thickness of 100 mm and
R -value of 4,75 m²·K/W. Base materials/Ancillary materials
D
The main materials are phenolic (PF) resin (between 70-80%)
For the placing on the market of the product in the European with added catalyst and additives (between 15-20%). Phenolic
Union/European Free Trade Association (EU/EFTA) (with the rigid foam onto a facing material (between 5-10%) is formed by
exception of Switzerland) Regulation (EU) No. 305/2011 (CPR) the chemical reaction of these materials and adding a blowing
applies. The product needs a declaration of performance taking agent with no ozone depletion potential (ca. 5%). Due to the
into consideration EN 13166:2012+A2:2016 - Thermal closed-cell structure (conform EN 13166), the blowing agent
insulation products for buildings - Factory made phenolic foam remains in the foam.
(PF) products - Specification and the CE-marking. In the current REACH regulations, phenolic foam insulation
For the application and use the respective national provisions products are considered 'articles' and are exempt from the
apply. requirements of Article 57 and 59(1) of REACH Regulation (EC)
No 1907/2006. These products are not classified as 'hazardous
Application products' according to any current legislation, and can hence
Due to its high insulating value, Kooltherm® K12 D is suitable be declared as follows:
for use as insulation for framing systems. - This article contains substances listed in the candidate list
(date: 19.01.2021) exceeding 0.1 percentage by mass: no.
Technical Data - This article contains other carcinogenic, mutagenic, reprotoxic
(CMR) substances in categories 1A or 1B which are not on the
Constructional data
candidate list, exceeding 0.1 percentage by mass: no.
Name Value Unit
- Biocide products were added to this construction product or it
Compressive strength acc. to EN 13166 ≥ 100 kPa has been treated with biocide products (this then concerns a
Thermal conductivity λd acc. to EN 13166 for d treated product as defined by the (EU) Biocidal Products
0.021W/(mK)
= 20 – 44 mm Regulation No. 528/2012 (BPR): no.
Thermal conductivity λd acc. to EN 13166 for d
0.021W/(mK)
= 45 – 120 mm The chemical functional group of the additives used in the resin
is that of non-ionic surfactants.
Thermal conductivity λd acc. to EN 13166 for d
0.021W/(mK)
= 121 – 159 mm
Reference service life
Technical parameters not included are modulus of elasticity as The reference service life is not to be declared in this EPD as it
well as sound absorption (not relevant for this application) and does not cover the use stage.
creep (not placed under permanent load).
LCA: Calculation rules
· A3, manufacturing, including provision of all materials,
Declared Unit products and energy, packaging processing and its transport,
The declared unit (1 m²) and conversion factors are listed in the as well as waste processing up to the end-of-waste state or
table below. disposal of final residues during the product stage.
Declared unit
The construction process stage includes:
Name Value Unit
· A4 transport to the building site;
Declared unit 1 m2 · A5 installation in the building
Gross density 35 kg/m3 including provision of all materials, products and energy, as well
conversion factor [Mass/Declared Unit] ( in kg/m² ) 3.5 - as waste processing up to the end-of-waste state or disposal of
final residues during the construction process stage.
Grammage 3.5 kg/m2
Layer thickness 0.1 m The end-of-life stage is a mandatory information module and it
covers:
System boundary · C1 de-construction, demolition;
Type of EPD: according to EN 15804: · C2 transport to waste processing;
cradle to gate with options, modules C1–C4, and module D · C3 waste processing for reuse, recovery and/or recycling;
(A1–A3, C, D and additional modules: A4,A5). · C4 disposal (not applicable for this EPD) including provision
According to PCR Part A: and all transport, provision of all materials, products and related
1a) declaration of one specific product from one plant of one energy and water use.
manufacturer.
Environmental burden of the incineration (R1 > 60%) of the
The product stage is a mandatory information module and it product at the end-of-life stage are assigned to the product
covers: system (C3); resulting potential credits for thermal and electrical
· A1, raw material extraction and processing, processing of energy from energy substitution are declared in module D.
secondary material input (e.g. recycling processes),
· A2, transport to the manufacturer, Renewable electricity sources for manufacturing
2 Environmental Product Declaration - Kingspan Insulation B.V. - Kooltherm® K12 D
All electricity used during production comes from renewable with Service Packs 39 GaBi ts is used.
sources.
By generating energy on-site with solar panels and with Geographic Representativeness
procured energy from fully certified renewable sources. Land or region, in which the declared product system is
Following the global Net Zero Energy strategy from Kingspan manufactured, used or handled at the end of the product´s
Group plc. lifespan: Europe
Period under review
Comparability
The input data for raw material production and the consumption
Basically, a comparison or an evaluation of EPD data is only
of process energy on the manufacturing facility was measure
possible if all the data sets to be compared were created
data during January 1st 2019 to December 31st 2019, i.e.
according to EN 15804 and the building context, respectively
collected over a 12 month period.
the product-specific characteristics of performance, are taken
into account. Background data from GaBi software-system
Background database
version 9 with Service Packs 39 GaBi ts is used.
Background data from GaBi software-system version 9
LCA: Scenarios and additional technical information
Within A1-A3 the following packaging of the final product is
Characteristic product properties of biogenic carbon included:
The total mass of biogenic carbon containing materials is less Polyethylene cover and wrap: 0,06 kg/m²
than 5 % of the total mass of the product and accompanying Others (mainly Expanded Polystyrene skid): 0,02 kg/m²
packaging. The recycling of the packaging is considered in A5.
End of life (C1-C4)
Technical information
The assumptions for C1 are: diesel driven excavator (100 kW;
The following technical information is a basis for the declared
0.2 litre fuel per ton excavated material).
modules or can be used for developing specific scenarios in the
The assumptions for C2 are: Truck Euro 6, diesel driven, 26-28
context of a building assessment.
t gross weight, assumed distance 50 km
Transport to the building site (A4)
Name Value Unit
Name Value Unit
Collected as mixed construction waste 3.5 kg
Litres of fuel 0.0103 l/100km
Energy recovery 3.5 kg
Transport distance 100 km
R1-value of waste incineration plant >60 %
Gross density of products transported 35 kg/m3
Reuse, recovery and/or recycling potentials (D), relevant
Installation into the building (A5) scenario information
Name ValueUnit
Waste incineration with energy recuperation is assumed as
Output substances following waste treatment on
0.08 kg end-of-life scenario
site packaging material
3 Environmental Product Declaration - Kingspan Insulation B.V. - Kooltherm® K12 D
LCA: Results
Disclaimer:
EP-freshwater: This indicator has been calculated as 'kg P eq' as required in the characterization model (EUTREND model, Struijs et
al., 2009b, as implemented in ReCiPe; http://eplca.jrc.ec.europa.eu/LCDN/developerEF.xhtml)
DESCRIPTION OF THE SYSTEM BOUNDARY (X = INCLUDED IN LCA; ND = MODULE OR INDICATOR NOT DECLARED; MNR =
MODULE NOT RELEVANT)
Benefits and
Construction loads beyond
Product stage Use stage End-of-life stage
process stage the system
boundaries
la ire ta m w a Ry lp p u s tro p s n a rT g n iru tc a fu n a M e h t m o rf tro p s n a rTe tis e h t o t e ta g y lb m e s s A e s U e c n a n e tn ia M ria p e R tn e m e c a lp e R tn e m h s ib ru fe R y g re n e la n o ita re p Oe s u re ta w la n o ita re p Oe s u n o itc u rts n o c -e Dn o itilo m e d tro p s n a rT g n is s e c o rp e ts a W la s o p s iD -e s u e R-y re v o c e R-g n ilc y c e Rla itn e to p
A1 A2 A3 A4 A5 B1 B2 B3 B4 B5 B6 B7 C1 C2 C3 C4 D
X X X X X MND MND MNR MNR MNR MND MND X X X X X
RESULTS OF THE LCA - ENVIRONMENTAL IMPACT according to EN 15804+A2: 1 m2 100 mm thickness
Parameter Unit A1-A3 A4 A5 C1 C2 C3 C4 D
GWP-total kg CO 2 eq 7.47E+00 2.98E-02 2E-01 2.25E-03 1.49E-02 7.73E+00 0 -3.33E+00
GWP-fossil kg CO 2 eq 7.62E+00 2.96E-02 2E-01 2.25E-03 1.48E-02 7.73E+00 0 -3.32E+00
GWP-biogenic kg CO 2 eq -2.32E-01 -1.8E-04 -3.63E-06 -1.59E-07 -8.99E-05 3.47E-04 0 -6.44E-03
GWP-luluc kg CO 2 eq 7.73E-02 4.52E-04 7.2E-06 7.64E-08 2.26E-04 7.47E-05 0 -2.26E-03
ODP kg CFC11 eq 1.31E-08 3.59E-18 5.97E-17 2.16E-19 1.8E-18 9.26E-16 0 -3.4E-14
AP mol H+ eq 1.84E-02 3.49E-05 2.76E-05 1.07E-05 1.75E-05 4.61E-03 0 -6.28E-03
EP-freshwater kg P eq 2.63E-05 1.43E-07 1.05E-08 4E-10 7.13E-08 1.58E-07 0 -4.37E-06
EP-marine kg N eq 4.54E-03 1.08E-05 7.28E-06 5E-06 5.38E-06 2.21E-03 0 -1.44E-03
EP-terrestrial mol N eq 4.58E-02 1.26E-04 1.2E-04 5.47E-05 6.3E-05 2.55E-02 0 -1.55E-02
kg NMVOC
POCP 1.95E-02 2.81E-05 2.09E-05 1.42E-05 1.4E-05 5.69E-03 0 -4.14E-03
eq
ADPE kg Sb eq 6.36E-06 2.06E-09 8.6E-10 5.92E-11 1.03E-09 1.58E-08 0 -5.19E-07
ADPF MJ 2.01E+02 3.94E-01 7.91E-02 3.05E-02 1.97E-01 2.09E+00 0 -5.75E+01
m3 world eq
WDP 1.28E+00 6.38E-04 2.08E-02 3.93E-06 3.19E-04 7.58E-01 0 -3.09E-01
deprived
GWP = Global warming potential; ODP = Depletion potential of the stratospheric ozone layer; AP = Acidification potential of land and water; EP =
Eutrophication potential; POCP = Formation potential of tropospheric ozone photochemical oxidants; ADPE = Abiotic depletion potential for non-fossil
resources; ADPF = Abiotic depletion potential for fossil resources; WDP = Water (user) deprivation potential)
RESULTS OF THE LCA - INDICATORS TO DESCRIBE RESOURCE USE according to EN 15804+A2: 1 m2 100 mm thickness
Parameter Unit A1-A3 A4 A5 C1 C2 C3 C4 D
PERE MJ 3.57E+01 2.29E-02 1.53E-02 8.97E-05 1.14E-02 2.78E-01 0 -1.17E+01
PERM MJ 0 0 0 0 0 0 0 0
PERT MJ 3.57E+01 2.29E-02 1.53E-02 8.97E-05 1.14E-02 2.78E-01 0 -1.17E+01
PENRE MJ 1.06E+02 3.94E-01 7.92E-02 3.05E-02 1.97E-01 9.79E+01 0 -5.75E+01
PENRM MJ 9.58E+01 0 0 0 0 -9.58E+01 0 0
PENRT MJ 2.01E+02 3.94E-01 7.92E-02 3.05E-02 1.97E-01 2.09E+00 0 -5.75E+01
SM kg 0 0 0 0 0 0 0 0
RSF MJ 0 0 0 0 0 0 0 0
NRSF MJ 0 0 0 0 0 0 0 0
FW m3 5.71E-02 3.87E-05 4.94E-04 1.66E-07 1.93E-05 1.79E-02 0 -1.37E+02
PERE = Use of renewable primary energy excluding renewable primary energy resources used as raw materials; PERM = Use of renewable primary
energy resources used as raw materials; PERT = Total use of renewable primary energy resources; PENRE = Use of non-renewable primary energy
excluding non-renewable primary energy resources used as raw materials; PENRM = Use of non-renewable primary energy resources used as raw
materials; PENRT = Total use of non-renewable primary energy resources; SM = Use of secondary material; RSF = Use of renewable secondary fuels;
NRSF = Use of non-renewable secondary fuels; FW = Use of net fresh water
RESULTS OF THE LCA – WASTE CATEGORIES AND OUTPUT FLOWS according to EN 15804+A2:
1 m2 100 mm thickness
Parameter Unit A1-A3 A4 A5 C1 C2 C3 C4 D
HWD kg 8.87E-05 2.2E-08 3.71E-10 3.24E-12 1.1E-08 1.33E-09 0 -2.37E-08
NHWD kg 3.18E-01 3.21E-05 1.93E-02 1.82E-07 1.6E-05 3.88E-02 0 -2.49E-02
RWD kg 2.76E-03 5.35E-07 3.64E-06 3.51E-08 2.68E-07 9.39E-05 0 -4.65E-03
CRU kg 0 0 0 0 0 0 0 0
MFR kg 0 0 0 0 0 0 0 0
MER kg 0 0 7.99E-02 0 0 3.5E+00 0 0
4 Environmental Product Declaration - Kingspan Insulation B.V. - Kooltherm® K12 D
EEE MJ 0 0 4.43E-01 0 0 1.34E+01 0 0
EET MJ 0 0 7.98E-01 0 0 2.39E+01 0 0
HWD = Hazardous waste disposed; NHWD = Non-hazardous waste disposed; RWD = Radioactive waste disposed; CRU = Components for re-use;
MFR = Materials for recycling; MER = Materials for energy recovery; EEE = Exported electrical energy; EET = Exported thermal energy
RESULTS OF THE LCA – additional impact categories according to EN 15804+A2-optional:
1 m2 100 mm thickness
Parameter Unit A1-A3 A4 A5 C1 C2 C3 C4 D
Disease
PM 1.8E-07 2.01E-10 3.77E-10 1.2E-10 1E-10 1.32E-08 0 -5.32E-08
incidence
IR kBq U235 eq 4.58E-01 7.84E-05 4.82E-04 5.13E-06 3.92E-05 1.46E-02 0 -7.63E-01
ETP-fw CTUe 7.15E+01 2.65E-01 5.6E-02 2.06E-02 1.33E-01 7.07E-01 0 -1.28E+01
HTP-c CTUh 7.66E-09 5.32E-12 4.28E-12 3.5E-13 2.66E-12 1.2E-10 0 -2.34E-09
HTP-nc CTUh 9.96E-08 2.14E-10 3.14E-10 1.22E-11 1.07E-10 1.39E-09 0 -1.18E-08
SQP SQP 3.56E+01 1.78E-01 1.99E-02 7.99E-05 8.89E-02 4.09E-01 0 -8.66E+00
PM = Potential incidence of disease due to PM emissions; IR = Potential Human exposure efficiency relative to U235; ETP-fw = Potential comparative
Toxic Unit for ecosystems; HTP-c = Potential comparative Toxic Unit for humans (cancerogenic); HTP-nc = Potential comparative Toxic Unit for humans
(not cancerogenic); SQP = Potential soil quality index
Disclaimer 1 – for the indicator IR
This impact category deals mainly with the eventual impact of low dose ionizing radiation on human health of the nuclear fuel cycle. It
does not consider effects due to possible nuclear accidents, occupational exposure nor due to radioactive waste disposal in
underground facilities. Potential ionizing radiation from the soil, from radon and from some construction materials is also not measured
by this indicator.
Disclaimer 2 – for the indicators ADPE, ADPF, WDP, ETP-fw, HTP-c, HTP-nc, SQP
The results of this environmental impact indicator shall be used with care as the uncertainties on these results are high or as there is
limited experienced with the indicator.
Factors for different thicknesses
The LCA results for the insulation material declared in this EPD refer to a product with a thickness of 100 mm. To enable the user of the
EPD to calculate the results for different thicknesses the factors in the following table can be used for the calculation. For modules A1-
A3, C3 and D the LCA results in chapter 5 have to be multiplied with these factors.
This EPD was created using a software tool.
References
EN 13166 CPR
EN 13166:2012+A2:2016: Thermal insulation products for Regulation (EU) No. 305/2011 of the European Parliament and
buildings. Factory made phenolic foam (PF) products. of the Council of 9 March 2011 laying down harmonised
Specification condition for the marketing of construction products and
repealing Council Directive 89/106/EC
EN 15804+A2
EN15804/A2: Sustainability of construction works - GaBi ts
Environmental product declarations - Core rules for the product thinkstep AG: Leinfelden-Echterdingen GaBi Software- System
category of construction products, 2019 and Database for Life Cycle Engineering 1992- 2019
BPR IBU 2016
Regulation (EU) No 528/2012 of the European Parliament and IBU (2016): General Programme Instructions for the
of the Council of 22 May 2012 concerning the making available Preparation of EPDs at the Institut Bauen und Umwelt e.V.,
on the market and use of biocidal products Version 1.1 Institut Bauen und Umwelt e.V., Berlin, www.ibu-
epd.de
5 Environmental Product Declaration - Kingspan Insulation B.V. - Kooltherm® K12 D
PCR 2017, Part B
ISO 14025 Institut Bauen und Umwelt e.V., Berlin (pub.): Product Category
EN ISO 14025:2011-10 - Environmental labels and declarations Rules for Construction Products from the range of
— Type III environmental declarations — Principles and Environmental Product Declarations of Institut Bauen und
procedures Umwelt (IBU), Part B: Requirements on the EPD for insulating
materials made of foam plastics.June 2017
LCA-tool
Kingspan LCA tool, version 1.0. IBU-KSI-202001-LT1-EN. REACH
Developed by Sphera Solutions GmbH (formely Thinkstep Regulation (EC) No 1907/2006 of the European Parliament and
GmbH) of the Council on the Registration, Evaluation, Authorisation
and Restriction of Chemicals (REACH)
PCR Version 1.7, Part A https://echa.europa.eu/candidate-list-table; accessed 19th of
Institut Bauen und Umwelt e.V., Berlin (pub.): Product Category January 2021, 211 substances listed.
Rules for Building-Related Products and services, Part A:
Calculation Rules for the Life Cycle Assessment and Renewable Energy Certificate
Requirements on the Project Report , March 2018 Towarowa Gielda Energii S.A.: Guarantees of origin Document
ID: RGP_ACTBV_2019-12-31_0720
6 Environmental Product Declaration - Kingspan Insulation B.V. - Kooltherm® K12 D
Publisher
Institut Bauen und Umwelt e.V. +49 (0)30 3087748- 0
Hegelplatz 1 info@ibu-epd.com
10117 Berlin www.ibu-epd.com
Germany
Programme holder
Institut Bauen und Umwelt e.V. +49 (0)30 3087748- 0
Hegelplatz 1 info@ibu-epd.com
10117 Berlin www.ibu-epd.com
Germany
Author of the Life Cycle Assessment
Kingspan Insulation B.V. +31 (0) 543 543 210
Lingewei 8 info@kingspaninsulation.nl
4004LL Tiel www.kingspan.com
Netherlands
Owner of the Declaration
Kingspan Insulation B.V. +31 (0) 543 543 210
Lingewei 8 info@kingspaninsulation.nl
4004LL Tiel www.kingspan.com
Netherlands
7 Environmental Product Declaration - Kingspan Insulation B.V. - Kooltherm® K12 D
