ENVIRONMENTAL PRODUCT DECLARATION
as per ISO 14025 and EN 15804+A2
Owner of the Declaration Kingspan Insulation B.V.
Publisher Institut Bauen und Umwelt e.V. (IBU)
Programme holder Institut Bauen und Umwelt e.V. (IBU)
Declaration number EPD-KSI-20220298-LT2-EN
Issue date 25.11.2022
Valid to 24.11.2027
Therma™ TR26 / Therma™ TT46 / Therma™ TR26 ML
Kingspan Insulation B.V.
www.ibu-epd.com | https://epd-online.com
General Information
Kingspan Insulation B.V. Therma™ TR26 / Therma™ TT46 / Therma™ TR26
ML
Programme holder Owner of the declaration
IBU – Institut Bauen und Umwelt e.V. Kingspan Insulation B.V.
Hegelplatz 1 Lingewei 8
10117 Berlin 4004LL Tiel
Germany Netherlands
Declaration number Declared product / declared unit
EPD-KSI-20220298-LT2-EN Therma™ TR26 / Therma™ TT46 / Therma™ TR26 ML
1m2, 120mm thickness, R = 5,45 m2.K/W
D
This declaration is based on the product category rules: Scope:
Insulating materials made of foam plastics, 01.08.2021 The insulation materials Therma™ TR26 / TR26 ML / TT46 are produced
(PCR checked and approved by the SVR) by Kingspan Insulation at the manufacturing facilities in Winterswijk (the
Netherlands), Burkhardtsdorf (Germany) and Kankaanpää (Finland). This
EPD is based on weighted averages which have been determined on the
Issue date basis of the single values originating from the different Kingspan Insulation
factories.
25.11.2022
Therma™ TR26 / TR26 ML is an insulation board with a rigid thermoset
polyisocyanurate (PIR) fibre free insulation core, faced on both sides with a
Valid to
low emissivity composite foil. Therma™ TR26 / TR26 ML is used as
24.11.2027 thermal insulation under mechanically fixed or non-fixed ballasted roofing
systems.
Therma™ TT46 Tapered Roof Board is an insulation board with a rigid
thermoset PIR fibre free insulation core, faced on both sides with a low
emissivity composite foil. Therma™ TT46 Tapered Roof Board is used as
thermal insulation under mechanically fixed or non-fixed ballasted roofing
systems and enhances water drainage from flat roofs.
In order to enable the user of the EPD to calculate the LCA results for
different thicknesses, the EPD contains the respective calculation rules.
The owner of the declaration shall be liable for the underlying information
and evidence; the IBU shall not be liable with respect to manufacturer
Dipl.-Ing. Hans Peters
information, life cycle assessment data and evidences.
(Chairman of Institut Bauen und Umwelt e.V.)
The EPD was created according to the specifications of EN 15804+A2. In
the following, the standard will be simplified as EN 15804.
Verification
The standard EN 15804 serves as the core PCR
Independent verification of the declaration and data according to ISO
14025:2011
internally X externally
Florian Pronold Vito D'Incognito,
(Managing Director Institut Bauen und Umwelt e.V.) (Independent verifier)
1 Environmental Product Declaration - Kingspan Insulation B.V. - Therma™ TR26 / Therma™ TT46 / Therma™ TR26 ML
Product
Performance data of the product in accordance with the
Product description/Product definition declaration of performance with respect to its essential
Therma™ TR26, Therma™ TR26 ML and Therma™ TT46 Roof characteristics according to EN 13165 - Thermal insulation
Boards are insulation boards with a rigid thermoset products for buildings - Factory made rigid polyurethane foam
polyisocyanurate (PIR) fibre free insulation core, faced on both (PU) products - Specification
sides with a low emissivity composite foil. The products are The declaration of performance of the product can be found at
available in variable thicknesses from 20 mm up to 215 mm. www.kingspan.com.
This EPD is based on a thickness of 120 mm and R -value of
D
Base materials/Ancillary materials
5,45 m²·K/W.
For the placing on the market of the product in the European The product contains approximately 3,3 kg/m2 polyurethane
Union/European Free Trade Association (EU/EFTA) (with the rigid foam and 0,3 kg/m2 multi-layer aluminium facings. The
exception of Switzerland) Regulation (EU) No. 305/2011 (CPR) main materials of the polyurethane foam are MDI (between 57-
applies. The product needs a declaration of performance taking 62 %), polyol (between 27-32 %) and a blowing agent (between
into consideration EN 13165 - Thermal insulation products for 5-6 %). Due to the closed cell structure (conform EN 13165),
buildings - Factory made polyurethane foam (PU) products - the blowing agent remains in the foam. Water, flame retardants
specification and the CE-marking. For the application and use and additives are added (between 4-8 %).
the respective national provisions apply.
In the current REACH regulations, polyurethane foam insulation
Application products are considered 'articles' and are exempt from the
Therma™ TR26 / Therma™ TR26 ML Roof Board is used as requirements of Articles 57 and 59(1) of REACH Regulation
thermal insulation under mechanically fixed or non-fixed (EC) No 1907/2006. These products are not classified as
ballasted roofing systems. 'hazardous products' according to any current legislation, and
can hence be declared as follows:
Therma™ TT46 Tapered Roof Board is used as thermal
insulation under mechanically fixed or non-fixed ballasted - This article contains substances listed in the
roofing systems and enhances water drainage from flat roofs. candidate list (date: 31.08.2022) exceeding 0.1 percentage by
mass: no.
Technical Data
- This article contains other carcinogenic, mutagenic, reprotoxic
Constructional data (CMR) substances in categories 1A or 1B which are not on the
candidate list, exceeding 0.1 percentage by mass: no.
Name Value Unit
Thermal conductivity according to EN
0.022 W/(m.K) - Biocide products were added to this construction product or it
13165
has been treated with biocide products (this then concerns a
Reaction to fire according to EN E treated product as defined by the (EU) Biocidal Products
13165 Regulation No. 528/2012
Compressive strength according to CS(10\Y) (BPR): no.
EN 13165 120/150
Reference service life
Thickness tolerance according to EN
13165 T2-T3 The reference service life is not to be declared in this EPD as it
does not cover the use stage.
LCA: Calculation rules
Declared Unit The environmental impacts have been calculated per plant over
The declared unit (1 m²) and conversion factors are listed in the the calendar year 2021. Based on the one-year production
table below. volume of Therma™ TR26, Therma™ TR26 ML and Therma™
Declared unit TT46 per plant, the individual environmental impacts are
weighted.
Name Value Unit
Declared unit 1 m2 The products Therma™ TR26, Therma™ TR26 ML and
Gross density 30 kg/m3 Therma™ TT46 are grouped because they have the same
Grammage 3.6 kg/m2 composition.
Layer thickness 0.12 m
The shape of both products differs, as the Therma™ TR26 /
conversion factor [Mass/Declared Unit] ( in kg/m² ) 3.6 Therma™ TR26 ML is a flat product and the Therma™ TT46 is
This EPD is based on a weighted average of the annual a tapered product. The EPD is studied for a common product
production volume of three factories producing the products thickness of 120 mm. Multiplication factors are included to
Therma™ TR26, Therma™ TR26 ML and Therma™ TT46. calculate impacts for other product thicknesses within the range
of 20 to 200 mm.
The scope of this EPD is the thermal insulation products
Therma™ TR26, Therma™ TR26 ML and Therma™ TT46 as Other declared units are allowed if the conversion is shown
produced by Kingspan Insulation at the manufacturing facilities transparently.
in Winterswijk (the Netherlands), Burkhardtsdorf (Germany) and
Kankaanpää (Finland). For IBU core EPDs (where clause 3.6 is part of the EPD): for
average EPDs, an estimate of the robustness of the LCA
2 Environmental Product Declaration - Kingspan Insulation B.V. - Therma™ TR26 / Therma™ TT46 / Therma™ TR26 ML
values must be made, e.g. concerning the variability of the Environmental burden of the incineration (R1 > 60 %) of the
production process, geographical representativeness and the product at the end-of-life stage are assigned to the product
influence of background data and preliminary products system (C3); resulting potential credits for thermal and electrical
compared to the environmental impacts caused by the actual energy from energy substitution are declared in module D.
production.
Geographic Representativeness
Land or region, in which the declared product system is
System boundary manufactured, used or handled at the end of the product´s
The type of EPD according to EN 15804 is: lifespan: Europe
cradle to gate with options, modules C1–C4, and
module D (A1–A3, C, D and additional modules:
A4, A5). Comparability
Basically, a comparison or an evaluation of EPD data is only
The product stage is a mandatory information module and it possible if all the data sets to be compared were created
covers: according to EN 15804 and the building context, respectively
· A1, raw material extraction and processing, processing of the product-specific characteristics of performance, are taken
secondary material input (e.g. recycling processes), into account.
· A2, transport to the manufacturer,
· A3, manufacturing, including provision of all materials, Background database
products and energy, packaging processing and its transport, Background data from GaBi ts Version 10 is used with GaBi
as well as waste processing up to the end-of-waste state or data sets CUP2022.1.
disposal of final residues
during the product stage.
The construction process stage includes: Factors for different thicknesses
· A4 transport to the building site; The LCA results for the insulation material declared in
· A5 installation in the building including provision of all this EPD refer to a product with a thickness of 120 mm.
materials, products and energy, as well as waste processing up To enable the user of the EPD to calculate the results for
to the end-of waste state or disposal of final residues during the different thicknesses the factors in the following
construction process stage. table can be used for the calculation. The LCA results in
chapter 5 have to be
The end-of-life stage is a mandatory information module and it multiplied by these factors.
covers:
· C1 de-construction, demolition; The scaling factors
· C2 transport to waste processing; are applicable for the complete product, where the multi-layer
· C3 waste processing for reuse, recovery and/or recycling; aluminium
· C4 disposal (not applicable for this EPD) including provision facings are for all product thicknesses equal and the foam
and all transport, provision of all materials, products and related inputs are scaling
energy and water use. upwards and downwards with other product thicknesses.
LCA: Scenarios and additional technical information
Characteristic product properties of biogenic carbon Manufacturing (A3)
The total mass of biogenic carbon containing materials is less A polyethylene packaging foil is used. The products are
than 5 % of the total mass of the product and accompanying transported either on EPS skids or on wooden pallets.
packaging.
Note: 1 kg of biogenic carbon is equivalent to 44/12 kg of CO 2. Within Module A3 the following packaging of the final product is
included:
- Polyethylene cover and wrap: 0,051 kg/m²
Technical information - Expanded Polystyrene skid: 0,031 kg/m²
The following technical information is a basis for the - Wooden pallet: 0,003 kg/m²
declared modules or can be used for developing
Transport to the building site (A4)
specific scenarios in the context of a building
assessment.
3 Environmental Product Declaration - Kingspan Insulation B.V. - Therma™ TR26 / Therma™ TT46 / Therma™ TR26 ML
Name Value Unit The same holds for a service life declared by the manufacturer.
Corresponding information related to in-use conditions needs
Litres of fuel 0.0103 l/100km
not be provided if a service life taken from the list of service life
Transport distance 100 km
by BNB is declared.
Gross density of products transported 30 kg/m3
Installation into the building (A5) End of life (C1-C4)
The assumptions for C1 are: diesel-driven excavator (100 kW;
Name ValueUnit
0.2 litre fuel per ton excavated material). The assumptions for
Total output substances following waste treatment
0.085 kg C2 are: Truck Euro 6, diesel driven, 26-28 t gross weight,
on-site packaging material
assumed distance 50 km.
The recycling of the packaging is considered in A5 Name ValueUnit
Collected as mixed construction waste 3.6 kg
Energy recovery 3.575 kg
In case a reference service life according to applicable ISO
standards is declared then the assumptions and in-use Recycling (aluminium content of the multi-layer
0.025 kg
conditions underlying the determined RSL shall be declared. In aluminium facings)
addition, it shall be stated that the RSL applies to the reference Reuse, recovery and/or recycling potentials (D), relevant
conditions only. scenario information
Waste incineration with energy recuperation is assumed as an
end-of-life scenario
4 Environmental Product Declaration - Kingspan Insulation B.V. - Therma™ TR26 / Therma™ TT46 / Therma™ TR26 ML
LCA: Results
In Table 1 "Description of the system boundary", all declared modules shall be indicated with an "X"; all modules that are not declared
shall be indicated with "MND" (As default the modules B3, B4, B5 are marked as MNR – module not relevant). In the following tables,
columns can be deleted for modules that are not declared. Indicator values should be declared with three valid digits (eventually using
the exponential form (e.g. 1,23E-5 = 0,0000123). A uniform format should be used for all values of one indicator.
If several modules are not declared and therefore have been deleted from the table, the abbreviations for the indicators can be
replaced by the complete names, while the readability and clear arrangement should be maintained; the legends can then be deleted.
If due to relevant data gaps, an indicator cannot be declared in a robust way, then the abbreviation “IND” (indicator not declared)
should be used for this indicator.
• 0 - calculated value is 0
• 0 - value falls under the cut-off
• 0 - assumption which exclude any flows (e.g. exported
electricity A1-A3)
• IND – in cases where the inventory does not support
the methodological approach or the calculation of the
specific indicator IND shall be used.
If no reference service life is declared (see chapter 2.13 "Reference Service Life"), the LCA results of the modules B1-B2 and B6-B7
shall refer to a period of one year. This shall then be indicated as an explanatory text below the tables. In addition, the formula for the
quantification of such B-modules over the total life cycle shall be provided.
DESCRIPTION OF THE SYSTEM BOUNDARY (X = INCLUDED IN LCA; MND = MODULE OR INDICATOR NOT DECLARED; MNR
= MODULE NOT RELEVANT)
Benefits and
Construction loads beyond
Product stage Use stage End of life stage
process stage the system
boundaries
la ire ta m w a Ry lp p u s tro p s n a rT g n iru tc a fu n a M e h t m o rf tro p s n a rTe tis e h t o t e ta g y lb m e s s A e s U e c n a n e tn ia M ria p e R tn e m e c a lp e R tn e m h s ib ru fe R y g re n e la n o ita re p Oe s u re ta w la n o ita re p Oe s u n o itc u rts n o c -e Dn o itilo m e d tro p s n a rT g n is s e c o rp e ts a W la s o p s iD -e s u e R-y re v o c e R-g n ilc y c e Rla itn e to p
A1 A2 A3 A4 A5 B1 B2 B3 B4 B5 B6 B7 C1 C2 C3 C4 D
X X X X X MND MND MNR MNR MNR MND MND X X X X X
RESULTS OF THE LCA - ENVIRONMENTAL IMPACT according to EN 15804+A2: 1 m² 120 mm Therma™ TR26 / Therma™ TT46
Parameter Unit A1-A3 A4 A5 C1 C2 C3 C4 D
GWP-total kg CO 2 eq 1.01E+01 3.03E-02 2.16E-01 2.31E-03 1.51E-02 7.79E+00 0 -3.21E+00
GWP-fossil kg CO 2 eq 1.03E+01 3.01E-02 2.16E-01 2.3E-03 1.51E-02 7.63E+00 0 -3.19E+00
GWP-biogenic kg CO 2 eq -2.35E-01 -4.16E-05 1.18E-05 3.08E-06 -2.08E-05 1.66E-01 0 -1.59E-02
GWP-luluc kg CO 2 eq 6.7E-03 1.68E-04 2.57E-06 2.84E-08 8.4E-05 1.43E-05 0 -3.65E-04
ODP kg CFC11 eq 2.82E-11 1.81E-15 3.85E-14 1.41E-16 9.03E-16 5.77E-13 0 -2.05E-11
AP mol H+ eq 2.18E-02 3.11E-05 2.7E-05 1.07E-05 1.55E-05 4.55E-03 0 -4.91E-03
EP-freshwater kg P eq 4.66E-05 9E-08 9.73E-09 4.65E-10 4.5E-08 1.56E-07 0 -4.22E-06
EP-marine kg N eq 5.6E-03 1.02E-05 7.23E-06 5.1E-06 5.08E-06 2.2E-03 0 -1.19E-03
EP-terrestrial mol N eq 5.78E-02 1.21E-04 1.23E-04 5.58E-05 6.05E-05 2.53E-02 0 -1.27E-02
kg NMVOC
POCP 2.77E-02 2.74E-05 2.08E-05 1.45E-05 1.37E-05 5.64E-03 0 -3.35E-03
eq
ADPE kg Sb eq 1.14E-05 2.52E-09 9.4E-10 9.43E-11 1.26E-09 1.58E-08 0 -4.68E-07
ADPF MJ 2.67E+02 4.03E-01 7.99E-02 3.12E-02 2.01E-01 2.02E+00 0 -5.35E+01
m3 world eq
WDP 1.56E+00 2.7E-04 2.05E-02 4.28E-06 1.35E-04 7.72E-01 0 -3.51E-01
deprived
GWP = Global warming potential; ODP = Depletion potential of the stratospheric ozone layer; AP = Acidification potential of land and water; EP =
Eutrophication potential; POCP = Formation potential of tropospheric ozone photochemical oxidants; ADPE = Abiotic depletion potential for non-fossil
resources; ADPF = Abiotic depletion potential for fossil resources; WDP = Water (user) deprivation potential)
RESULTS OF THE LCA - INDICATORS TO DESCRIBE RESOURCE USE according to EN 15804+A2: 1 m² 120 mm Therma™
TR26 / Therma™ TT46
Parameter Unit A1-A3 A4 A5 C1 C2 C3 C4 D
PERE MJ 2.88E+01 2.29E-02 2.05E-02 1.18E-04 1.15E-02 3.54E-01 0 -1.52E+01
PERM MJ 0 0 0 0 0 0 0 0
PERT MJ 2.88E+01 2.29E-02 2.05E-02 1.18E-04 1.15E-02 3.54E-01 0 -1.52E+01
PENRE MJ 1.52E+02 4.04E-01 3.7E+00 3.12E-02 2.02E-01 1.14E+02 0 -5.35E+01
PENRM MJ 1.15E+02 0 -3.62E+00 0 0 -1.12E+02 0 0
PENRT MJ 2.68E+02 4.04E-01 7.99E-02 3.12E-02 2.02E-01 2.02E+00 0 -5.35E+01
SM kg 0 0 0 0 0 0 0 0
5 Environmental Product Declaration - Kingspan Insulation B.V. - Therma™ TR26 / Therma™ TT46 / Therma™ TR26 ML
RSF MJ 0 0 0 0 0 0 0 0
NRSF MJ 0 0 0 0 0 0 0 0
FW m3 7.19E-02 2.59E-05 4.87E-04 1.78E-07 1.3E-05 1.82E-02 0 -1.64E-02
PERE = Use of renewable primary energy excluding renewable primary energy resources used as raw materials; PERM = Use of renewable primary
energy resources used as raw materials; PERT = Total use of renewable primary energy resources; PENRE = Use of non-renewable primary energy
excluding non-renewable primary energy resources used as raw materials; PENRM = Use of non-renewable primary energy resources used as raw
materials; PENRT = Total use of non-renewable primary energy resources; SM = Use of secondary material; RSF = Use of renewable secondary fuels;
NRSF = Use of non-renewable secondary fuels; FW = Use of net fresh water
RESULTS OF THE LCA – WASTE CATEGORIES AND OUTPUT FLOWS according to EN 15804+A2:
1 m² 120 mm Therma™ TR26 / Therma™ TT46
Parameter Unit A1-A3 A4 A5 C1 C2 C3 C4 D
HWD kg 1.12E-07 1.93E-12 6.65E-12 1.03E-13 9.67E-13 2.76E-10 0 -6.62E-09
NHWD kg 2.85E-01 5.79E-05 1.94E-02 2.92E-06 2.89E-05 4.37E-02 0 -8.04E-02
RWD kg 2.94E-03 4.97E-07 3.32E-06 3.42E-08 2.49E-07 8.4E-05 0 -4.19E-03
CRU kg 0 0 0 0 0 0 0 0
MFR kg 0 0 0 0 0 2.54E-02 0 0
MER kg 0 0 8.66E-02 0 0 3.46E+00 0 0
EEE MJ 0 0 3.93E-01 0 0 1.32E+01 0 0
EET MJ 0 0 7.03E-01 0 0 2.36E+01 0 0
HWD = Hazardous waste disposed; NHWD = Non-hazardous waste disposed; RWD = Radioactive waste disposed; CRU = Components for re-use;
MFR = Materials for recycling; MER = Materials for energy recovery; EEE = Exported electrical energy; EET = Exported thermal energy
RESULTS OF THE LCA – additional impact categories according to EN 15804+A2-optional:
1 m² 120 mm Therma™ TR26 / Therma™ TT46
Parameter Unit A1-A3 A4 A5 C1 C2 C3 C4 D
Disease
PM 1.83E-07 1.79E-10 3.29E-10 1.21E-10 8.97E-11 1.27E-08 0 -4.27E-08
incidence
IR kBq U235 eq 3.52E-01 7.29E-05 4.56E-04 4.98E-06 3.64E-05 1.35E-02 0 -7.15E-01
ETP-fw CTUe 1.09E+02 2.8E-01 5.72E-02 2.17E-02 1.4E-01 6.96E-01 0 -1.21E+01
HTP-c CTUh 7.21E-09 5.64E-12 3.2E-12 4.01E-13 2.82E-12 5.21E-11 0 -6.3E-10
HTP-nc CTUh 6.13E-07 2.93E-10 3.24E-10 2.03E-11 1.46E-10 1.9E-09 0 -2.22E-08
SQP SQP 6.43E+01 1.39E-01 2.04E-02 8.6E-05 6.93E-02 4.26E-01 0 -9.22E+00
PM = Potential incidence of disease due to PM emissions; IR = Potential Human exposure efficiency relative to U235; ETP-fw = Potential comparative
Toxic Unit for ecosystems; HTP-c = Potential comparative Toxic Unit for humans (cancerogenic); HTP-nc = Potential comparative Toxic Unit for humans
(not cancerogenic); SQP = Potential soil quality index
Disclaimer 1 – for the indicator “Potential Human exposure efficiency relative to U235”.This impact category deals mainly with the
eventual impact of low dose ionizing radiation on human health of the nuclear fuel cycle. It does not consider effects due to possible
nuclear accidents, occupational exposure or to radioactive waste disposal in underground facilities. Potential ionizing radiation from the
soil, radon and from some construction materials is also not measured by this indicator.
Disclaimer 2 – for the indicators “abiotic depletion potential for non-fossil resources”, “abiotic depletion potential for fossil resources”,
“water (user) deprivation potential, deprivation-weighted water consumption”, “potential comparative toxic unit for ecosystems”,
“potential comparative toxic unit for humans – cancerogenic”, “Potential comparative toxic unit for humans - not cancerogenic”,
“potential soil quality index”. The results of this environmental impact indicator shall be used with care as the uncertainties on these
results are high as there is limited experienced with the indicator. This EPD was created using a software tool.
References
Biocidal Products Regulation No. 528/2012 (BPR) EN 15804:2012+A2:2019+AC:2021, Sustainability of
Regulation (EU) No 528/2012 of the European construction works — Environmental Product Declarations —
Parliament and of the Council of 22 May 2012 Core rules for the product category of construction products.
concerning the making available on the market and
use of biocidal products GaBi ts
thinkstep AG: Leinfelden-Echterdingen GaBi Software-
System and Database for Life Cycle Engineering 1992-
2019
CPR
Regulation (EU) No. 305/2011 of the European Parliament and
of the Council of 9 March 2011 laying down harmonised IBU 2021
condition for the marketing of construction products and Institut Bauen und Umwelt e.V.: General Instructions for the
repealing Council Directive EPD programme of Institut Bauen und Umwelt e.V., Version
89/106/EC 2.0, Berlin: Institut Bauen und Umwelt e.V., 2021
www.ibu-epd.com
EN 13165
EN 13165:2012+A2:2016: Thermal insulation products
for buildings. Factory made polyurethane foam (PU)
products. Specification
ISO 14025
EN 15804 EN ISO 14025:2011, Environmental labels and declarations —
6 Environmental Product Declaration - Kingspan Insulation B.V. - Therma™ TR26 / Therma™ TT46 / Therma™ TR26 ML
Type III environmental declarations — Principles and Rules for Construction Products from the range of
procedures. Environmental Product Declarations of Institut Bauen und
Umwelt (IBU), Part B: Requirements on the EPD for insulating
LCA-tool materials made of foam
Kingspan LCA tool, version 1.1. IBU-KSI-202001-LT1- plastics. January 2019
EN.
Developed by Sphera Solutions GmbH (formely REACH
Thinkstep GmbH) Regulation (EC) No 1907/2006 of the European
Parliament and of the Council on the Registration,
PCR Version 1.7, Part A Evaluation, Authorisation and Restriction of Chemicals
Institut Bauen und Umwelt e.V., Berlin (pub.): Product Category (REACH)
Rules for Building-Related Products and services, Part A: https://echa.europa.eu/candidate-list-table; accessed
Calculation Rules for the Life Cycle Assessment and 19th of January 2021, 211 substances listed.
Requirements on the Project Report according to EN The literature referred to in the Environmental Product
15804+A2:2019 Declaration must be listed in full.Standards already fully quoted
November 2021 in the EPD do not need to be listed here again.
The current version of PCR Part A and PCR Part B of the PCR
PCR 2017, Part B document on which they are based must be referenced.
Institut Bauen und Umwelt e.V., Berlin (pub.): Product Category
7 Environmental Product Declaration - Kingspan Insulation B.V. - Therma™ TR26 / Therma™ TT46 / Therma™ TR26 ML
Publisher
Institut Bauen und Umwelt e.V. +49 (0)30 3087748- 0
Hegelplatz 1 info@ibu-epd.com
10117 Berlin www.ibu-epd.com
Germany
Programme holder
Institut Bauen und Umwelt e.V. +49 (0)30 3087748- 0
Hegelplatz 1 info@ibu-epd.com
10117 Berlin www.ibu-epd.com
Germany
Author of the Life Cycle Assessment
Kingspan Insulation B.V. +31 (0) 543 543 210
Lingewei 8 info@kingspaninsulation.nl
4004LL Tiel www.kingspan.com
Netherlands
Owner of the Declaration
Kingspan Insulation B.V. +31 (0) 543 543 210
Lingewei 8 info@kingspaninsulation.nl
4004LL Tiel www.kingspan.com
Netherlands
8 Environmental Product Declaration - Kingspan Insulation B.V. - Therma™ TR26 / Therma™ TT46 / Therma™ TR26 ML
