ENVIRONMENTAL PRODUCT DECLARATION
as per ISO 14025 and EN 15804+A2
Owner of the Declaration
Programme holder Institut Bauen und Umwelt e.V. (IBU)
Publisher Institut Bauen und Umwelt e.V. (IBU)
Declaration number EPD-ACF-20220040-ICA1-EN
Issue date 07.12.2022
Valid to 06.12.2027
Amorim Wise Cork Pure UV
Amorim Cork Flooring S.A.
www.ibu-epd.com | https://epd-online.com
Umwelt Produktdeklaration Name des Herstellers – Name des Produkts
1. General Information
Amorim Cork Flooring, S.A. Amorim Wise Cork Pure UV
Programme holder Owner of the declaration
IBU – Institut Bauen und Umwelt e.V. Amorim Cork Flooring, S.A.
Panoramastr. 1 Rua do Ribeirinho, nº 202
10178 Berlin Apartado 13
Germany 4536 - 907 S. Paio Oleiros
Portugal
Declaration number Declared product / declared unit
EPD-ACF-20220040-ICA1-EN 1 m2 of Amorim Wise Cork Pure UV
This declaration is based on the product Scope:
category rules: The data on which the Life Cycle Assessment is based
Floor coverings, 02/2018 is from the manufacturing process of Amorim Wise
(PCR checked and approved by the SVR) Cork Pure UV taking place in one industrial unit of
Amorim Revestimentos (Oleiros) and is referred to the
year of 2020. For the construction, use, end of life
Issue date
stages and benefits and loads, data were estimated
07.12.2022
based on background research and Amorim Cork
Flooring supply chain downstream activities. Data
Valid to associated with the product’s maintenance was
06.12.2027 obtained through benchmark research.
The owner of the declaration shall be liable for the
underlying information and evidence; the IBU shall not
be liable with respect to manufacturer information, life
cycle assessment data and evidences.
The EPD was created according to the specifications
of EN 15804+A2. In the following, the standard will be
simplified as EN 15804.
Verification
The standard EN 15804 serves as the core PCR
Independent verification of the declaration and data
according to ISO 14025:2010
Dipl. Ing. Hans Peters internally x externally
(chairman of Institut Bauen und Umwelt e.V.)
Dr. Alexander Röder Matthias Klingler
(Managing Director Institut Bauen und Umwelt e.V.)) (Independent verifier)
2. Product
2.1 Product description/Product definition 2.2 Application
Amorim Wise Cork Pure UV has a natural cork Amorim Wise Cork Pure UV fits the most demanding
structure, that provides superior comfort and needs for commercial areas. This flooring product
environmental performance for commercial areas, with meets the requirements of the usage class 33 for
a genuine cork veneer decorative layer and UV varnish commercial use according to ISO 10874 standard.
finishing. This product is used as a floor covering for
commercial use, providing several physical 2.3 Technical Data
characteristics to the floor, such as stability, comfort, Relevant technical construction data for the product is
thermal and noise insulation, among others. referred to in the following table.
For the placing on the market of the product in the Constructional data
European Union/European Free Trade Association Name Value Unit
(EU/EFTA) (with the exception of Switzerland) Product thickness 4.06 mm
Regulation (EU) No. 305/2011 CPR applies. The Grammage 2170 g/m2
product needs a Declaration of Performance taking Abrasion Class 33 -
into consideration EN 14041: 2004/AC:2006 Resilient, Product Form Plank -
textile and laminate floor coverings - Essential Total thickness 4 mm
characteristics and the CE-marking. For the application Density 542 kg/m3
and use the respective national provisions apply.
2 Environmental Product Declaration Amorim Cork Flooring – Amorim Wise Cork Pure UV
2.6 Manufacture
Amorim Wise Cork Pure UV may also be produced The manufacturing process of Amorim Wise Cork Pure
and commercialized with different thicknesses, of 6 UV begins with cork granulate production, using cork
mm, having the same product composition and that was previously treated at Amorim Florestal.
production process, but a different weight per square
meter of 3.25 kg. Around 88 % of the granulated cork previously
produced is forwarded to an agglomeration process in
The Performance data of the product is in accordance which a melamine-urea-formaldehyde (MUF) resin is
with the Declaration of Performance with respect to its used to produce the agglomerated cork layer. This
Essential Characteristics according to EN layer is the inferior layer of the final product and
14041:2004/AC:2006 Resilient, textile and laminate constitutes most of the thickness of the product. The
floor coverings - Essential characteristics. remaining granulated cork, together with a polyvinyl
acetate (PVA) resin, is used to produce the genuine
2.4 Delivery status cork veneer, the decorative layer of the Amorim Wise
The dimensions of rectangular panels of Amorim Wise Cork Pure UV.
Cork Pure UV are declared in the following table.
The agglomerated cork layer and the decorative
genuine cork veneer, that compose the final product
structure are glued together using glue and adhesives
as binding agents. This unfinished product then follows
to a pressure and heat process, before going through
sanding.
The product is ultimately varnished with a base coat as
well as a top coat varnish and finished by an UV
(ultraviolet) drying process. The result of this process
The layers composing Amorim Wise Cork Pure UV are is then forwarded for the final cut of the pieces and
shown in the following table. ultimately packed and stored in the shipment
warehouse, ready for shipment.
2.5 Base materials/Ancillary materials
Components
The primary product components and materials of the
product are indicated as a percentage mass in the
following table.
The products include partial articles which contain
substances listed in the candidate list of REACH
Regulation 1907/2006/EC (date: 19.01.2021)
exceeding 0.1 percentage by mass: no
This product/article/at least one partial article contains 2.7 Environment and health during
other carcinogenic, mutagenic, reprotoxic (CMR) manufacturing
substances in categories 1A or 1B which are not on During the production process, the environmental and
the candidate list, exceeding 0.1 percentage by mass: health aspects are considered.
no. Air: The emission of particles and pollutants are
collected in filter systems and the levels are below the
Biocide products were added to this construction permissible limits.
product or it has been treated with biocide products Water: The product requires a low water consumption
(this then concerns a treated product as defined by the that is (totally) treated in an Industrial Waste Water
(EU) Ordinance on Biocide Products No. 528/2012): Treatment Plant (IWWTP).
no. Noise: Noise resulting from operation during the
production process is below the permissible limits.
3 Environmental Product Declaration Amorim Cork Flooring – Amorim Wise Cork Pure UV
manufacturer, considering the different use classes,
2.8 Product processing/Installation according to ISO 10874. The following table indicates
For heated floors, the temperature of the subfloor the expected service life for commercial use.
must not exceed 28ºC (82ºF).
In concrete subfloors, the installation should be made
not before 21 days after the complete curing of the
substrate. The heating phase has to begin with the
running temperature of 25ºC (78ºF) for 3 days. The
subfloor should be in place and cured for at least 60-90 2.13 Extraordinary effects
days.
Fire
During the installation, the temperature of the surface Fire performance according to EN 13501 – 1 (building
should not exceed 18ºC (65ºF) and should be kept for products) of Amorim Wise Cork Pure UV is Cfl-S1.
3 days after finishing the installation (for floors). Then
the temperature should be increased slowly to a max. Water
of 28ºC (82ºF) on the subfloor surface. There are no environmental impacts on water identified
in the use stage of the product since the product is
For the product installation, it is necessary to use an mainly composed of natural materials that are not
adhesive. Amorim WISE recommends adhesives that hazardous to water masses.
are specially developed for ease of use, safety and
quality of the application. Mechanical destruction
There is no potential harm to health and environment
2.9 Packaging known resulting from the mechanical destruction of the
Cork Pure coverings are delivered in packages product.
designed to protect the corners, edges and surface of
the product, under normal conditions of transport and 2.14 Re-use phase
handling (compliant with EN 12104). The product is mainly composed of cork. Waste from
Product tiles are wrapped in film and laid in cardboard the product can be reused in the process as a
boxes. Boxes are placed in wooden pallets and replacement for some of the raw materials. This type of
wrapped by film . flooring can also be reused, although its service life is
These packaging materials can be collected separately expected to be longer than the original warranty from
and recycled. the manufacturer. Regarding energy recovery, cork
Pallets can either be re-used (Euro pallets) or recycled can be incinerated in order to produce thermal energy
as wood. or electricity.
2.15 Disposal
2.10 Condition of use According to the European Waste Catalogue Directive
Amorim Wise Cork Pure UV flooring products have in the used floor covering can be classified in the main
their composition a significant amount of natural category “17 Construction and Demolition Waste
renewable raw materials, meaning that they have (including road construction)”. Considering the specific
stored about 3,5 kg CO 2/m² of product resulting from constitution of this floor covering, and assuming that
photosynthesis. the layers cannot be separated at the end of life, the
waste code applied is the following: 17 09 04 Mixed
2.11 Environment and health during use construction and demolition waste other than those
The following table indicates the information about mentioned in 17 09 01, 17 09 02 and 17 09 03.
safety properties.
These types of waste materials can be recovered
according to the European Waste Framework
Directive.
2.16 Further information
Other information can be found on the Amorim Wise
website or the website of the manufacturer Amorim
Cork Flooring
www.amorimwise.com
www.amorimcorkflooring.com
2.12 Reference service life
The expected service life of the product was
determined based on empirical experience of the
3. LCA: Calculation rules
3.1 Declared Unit Grammage 2.17 kg/m2
The declared unit is 1 m2 of installed floor covering
with the following characteristics:
Declared unit 3.2 System boundary
Name Value Unit Type of EPD: cradle to gate with options
Declared unit 1 m2
4 Environmental Product Declaration Amorim Cork Flooring – Amorim Wise Cork Pure UV
Modules A1-A3 Production: Include processes that 3.4 Cut-off criteria
provide materials, transport of the material to the All input and output flows have been considered at 100
manufacturing site, energy supply, product %, including all available data associated directly to
manufacturing and transport processes up to the the manufacture of the product included in the LCA
factory gate, as well as waste processing. Biogenic (i.e. all raw materials, electric and thermal power
carbon contained in the product and the packaging consumed, transports). Hence, the study complies with
materials is included in this module. the cut-off criteria of 1 % of renewable and non-
renewable primary energy usage and 1 % of the total
Module A4 Transport: Transport of the floor covering mass of that unit process.
from the factory gate to the place of installation
3.5 Background data
Module A5 Installation: Includes material losses For processes in which the producer has no influence
(offcuts) during the installation of the floor covering, or specific information, like the extraction of raw
use of adhesives and disposal of offcuts and recycling materials, end-of-life treatment and generic data from
of packaging material. the following main sources were considered:
- Ecoinvent 3.5
Module B2 Maintenance: includes provision of - PRé Consultants (SimaPro 9.1)
energy, for vacuum cleaning once a week, cleaning
agent and water consumption, for wet cleaning twice a 3.6 Data quality
year Specific data is referred to production of 2020. Data
The LCA results in this EPD are declared for a one- sets of processes from Ecoinvent database are
year usage. less than 4 years old. Data sets are based on literature
and average data from specific industrial units.
Regarding geographical coverage, average European
Module C1 De-construction: The floor covering is de- data and Portugal specific energy mix were used. In
constructed manually and no additional environmental cases where no average European data was available,
impact is caused. it was used the most approximate data set.
Considering these aspects, the data used in this study
Module C2 Transport: Includes transportation of the is considered of high quality.
postconsumer waste to the waste incineration plant or
to a landfill. 3.7 Period under review
The specific data collected from the manufacturer refer
Module C3 Waste processing and Module C4 to the year 2020.
Disposal, end-of-life scenarios are declared for:
· 40 % incineration in a waste incineration plant 3.8 Allocation
(WIP) and 60 % landfilling (Mixed scenario) Energy, raw materials, water, by-products, waste,
· 100 % incineration in a waste incineration plant wastewater and air emissions were allocated to this
(WIP) (Scenario 1) product using mass allocation (i.e. allocation based on
· 100 % landfilling (Scenario 2) the proportional mass of each of the products, when no
further subdivision of unit processes was deemed
Module D Benefits and Loads: Declares potential feasible.
benefits from all net flows given in module A5
(packaging material recycling) and C3 (for incineration,
and related energy substitution) that leave the product 3.9 Comparability
boundary system after having passed the end-of-waste Basically, a comparison or an evaluation of EPD data
state. is only possible if all the data sets to be compared
Module D is declared for each scenario separately. were created according to EN 15804 and the building
context, respectively the product-specific
3.3 Estimates and assumptions characteristics of performance, are taken into account.
CO2 intake due to photosynthesis associated to cork
was considered. Information on components Background data are taken from the SimaPro software
and average weight percentage of adhesives was (version 9.1) and from the Ecoinvent 3.5 database,
obtained from their technical data sheets. 2018.
4. LCA: Scenarios and additional technical information
Characteristic product properties Biogenic carbon content in
0.182 kg C
Information on biogenic Carbon accompanying packaging
The product is composed of 84 % of materials that Note: 1 kg biogenic Carbon is equivalent to 44/12 kg
contain biogenic carbon. Packaging material, which of CO .
2
represents 17 % of the packed finished product, that
also contains biogenic carbon is accounted for in this The following information refers to the declared
section. modules and is the basis for calculations or can
be used for further calculations. The indicated values
Information on describing the biogenic Carbon refer to the declared unit.
Content at factory gate
Name Value Unit Transport to the construction site (A4)
Biogenic carbon content in Name Value Unit
0.947 kg C
product Transport, freight, lorry 16-32 230 km
5 Environmental Product Declaration Amorim Cork Flooring – Amorim Wise Cork Pure UV
metric ton, euro4
Transport, freight, sea,
2000 km
transoceanic ship
Transport, freight, lorry 3,5-7.5
5 km
metric ton, euro4
Installation in the building (A5)
Name Value Unit
Auxiliary Contact adhesive 0.2 kg
Material loss 0.065 kg
Output substances following
waste treatment on site Packaging 0.46 kg
waste
Packaging waste is considered to be recycled and
installation waste are considered to be disposed in a
landfill.
Maintenance (B2)
Name Value Unit
Maintenance cycle (wet cleaning) 2 1/year
Maintenance cycle (vacuum
52 1/year
cleaning)
Electricity consumption 0.1 kWh
Water consumption 0.001 m3
Auxiliary (cleaning agent) 0.02 kg
Reference service life
Name Value Unit
Reference service life (according
15 a
to ISO 15686-1, -2, -7 and -8)
End of Life (C1-C4)
Name Value Unit
Landfilling 100 % (C4/2) 2.17 kg
Transportation from the
construction site (C2 and C2/1)
50 km
(for the incineration EoL - by lorry
16-32 metric tons, euro 4)
Transportation from the
construction site (C2 and C2/2)
50 km
(for the Landfilling EoL - by lorry
16-32 metric tons, euro 4)
Energy recovery (C3) (mixed
0.87 kg
scenarios)
Landfilling (C4) (mixed scenarios) 1.30 kg
For module C1, is considered that the floorcovering is
de-constructed manually with no additional
environmental impacts.
Reuse, recovery and/or recycling potentials (D),
relevant scenario information
For module D, which represents the benefits and loads
beyond the system boundary, the potential benefits
from modules A5 and C3 are declared, considering the
recycling of packaging material waste and energy
benefits (incineration EoL).
For the waste incineration combustion scenario in a
WIP (R1 > 0.6), energy recuperation is considered.
6 Environmental Product Declaration Amorim Cork Flooring – Amorim Wise Cork Pure UV
5. LCA: Results
The results for module B2 refer to a period of one year. For the calculation of the impact of B2 for a certain
service life the values for B2 have to be multiplied by the estimated service life in years.
For modules C2, C3 and C4 the results are presented considering:
- C2, C3, C4, D refer to 40 % incineration, 60 % landfilling (mixed scenario)
- C2/1,C3/1, D/1 refer to 100 % incineration (scenario 1)
- C2/2, C4/2 and D/2 refer to 100 % landfilling (scenario 2)
Information on un-declared modules:
Modules B3 - B7 are not declared, since the use stage is declared for 1 year.
Disclaimer: EP-freshwater: This indicator has been calculated as “kg P eq” as required in the characterization
model (EUTREND model, Struijs et al., 2009b, as implemented in ReCiPe;
http://eplca.jrc.ec.europa.eu/LCDN/developerEF.xhtml).
DESCRIPTION OF THE SYSTEM BOUNDARY (X = INCLUDED IN LCA; ND = MODULE OR INDICATOR NOT
DECLARED; MNR = MODULE NOT RELEVANT)
BENEFITS AND
CONSTRUCTI LOADS
PRODUCT STAGE ON PROCESS USE STAGE END OF LIFE STAGE BEYOND THE
STAGE SYSTEM
BOUNDARIES
7 Environmental Product Declaration Amorim Cork Flooring – Amorim Wise Cork Pure UV
lairetam
waR
ylppus tropsnarT
gnirutcafunaM
eht
morf
tropsnarT
etis
eht
ot
etag
ylbmessA esU
ecnanetniaM
riapeR
tnemecalpeR tnemhsibrufeR
ygrene
lanoitarepO esu
retaw
lanoitarepO esu
noitcurtsnoc-eD
noitilomed tropsnarT
gnissecorp
etsaW
lasopsiD -esueR -yrevoceR -gnilcyceR laitnetop
A1 A2 A3 A4 A5 B1 B2 B3 B4 B5 B6 B7 C1 C2 C3 C4 D
X X X X X ND X MNR MNR MNR ND ND X X X X X
RESULTS OF THE LCA - ENVIRONMENTAL IMPACT according to EN 15804+A2: 1 m2 Amorim Wise Cork
Pure UV
Core Indicator Unit A1-A3 A4 A5 B2 C1 C2 C2/1 C2/2 C3 C3/1 C4 C4/2 D D/1 D/2
- -
0.00E+ 1.40E+ 3.51E+ 2.23E+ 3.72E+ -8.93E-
GWP-total [kg CO2-Eq.] 2.46E+1.66E-19.38E-11.13E-1
0
1.80E-21.80E-21.80E-2
0 0 0 0 1
2.51E+1.84E-1
0 0
- -
1.67E+ 0.00E+ -4.79E-
GWP-fossil [kg CO2-Eq.]
0
1.66E-12.71E-11.10E-1
0
1.80E-21.80E-21.80E-21.60E-24.01E-21.74E-22.90E-21.52E+ 3.09E+
1
0 0
-
-4.43E- 0.00E+ 1.39E+ 3.47E+ 2.22E+ 3.70E+
GWP-biogenic [kg CO2-Eq.] 4.14E+7.52E-56.67E-1
3 0
4.28E-64.28E-64.28E-6
0 0 0 0
6.37E-15.94E-16.66E-1
0
0.00E+ -5.54E- -9.52E- -2.89E-
GWP-luluc [kg CO2-Eq.] 1.44E-26.79E-53.84E-48.00E-3
0
5.71E-65.71E-65.71E-62.64E-66.59E-68.01E-61.34E-5
3 3 3
0.00E+ -1.38E- -2.74E- -4.67E-
ODP [kg CFC11-Eq.] 1.82E-73.58E-83.20E-86.13E-9 4.14E-94.14E-94.14E-91.33E-93.33E-95.67E-99.46E-9
0 7 7 8
0.00E+ -9.76E- -1.96E- -3.17E-
AP [mol H+-Eq.] 1.23E-21.81E-33.38E-35.61E-4 9.07E-59.07E-59.07E-51.73E-44.32E-41.49E-42.49E-4
0 3 2 3
0.00E+ -1.31E- -2.96E- -2.03E-
EP-freshwater [kg PO4-Eq.] 5.76E-41.67E-51.19E-46.29E-5
0
1.42E-61.42E-61.42E-67.14E-61.79E-54.16E-66.93E-6
3 3 4
0.00E+ -1.81E- -3.43E- -7.37E-
EP-marine [kg N-Eq.] 2.19E-33.57E-43.06E-41.43E-4 3.07E-53.07E-53.07E-58.97E-52.24E-45.93E-49.89E-4
0 3 3 4
0.00E+ -1.93E- -3.62E- -7.97E-
EP-terrestrial [mol N-Eq.] 2.65E-23.96E-33.08E-31.11E-3 3.36E-43.36E-43.36E-48.64E-42.16E-35.33E-48.88E-4
0 2 2 3
0.00E+ -4.82E- -8.58E- -2.31E-
POCP [kg NMVOC-Eq.]8.32E-31.12E-31.08E-33.83E-4 9.54E-59.54E-59.54E-52.12E-45.29E-41.91E-43.19E-4
0 3 3 3
0.00E+ -1.79E- -2.66E- -1.22E-
ADPE [kg Sb-Eq.] 4.45E-63.27E-71.42E-62.70E-7 5.01E-85.01E-85.01E-82.38E-85.95E-82.37E-83.95E-8
0 6 6 6
- - -
2.65E+ 2.45E+ 4.69E+ 2.36E+ 0.00E+
ADPF [MJ] 2.74E-12.74E-12.74E-11.40E-13.50E-14.28E-17.14E-13.00E+ 6.31E+ 7.92E+
1 0 0 0 0
1 1 0
-
[m³ world-Eq 1.69E+ 0.00E+ -9.62E- -2.40E- -9.82E- -6.71E-
WDP 1.68E-22.81E-18.48E-2 1.90E-31.90E-31.90E-3 1.84E-23.06E-2 1.45E+
deprived] 0 0 3 2 1 1
0
GWP = Global warming potential; ODP = Depletion potential of the stratospheric ozone layer; AP = Acidification potential of land and water; EP =
Caption Eutrophication potential; POCP = Formation potential of tropospheric ozone photochemical oxidants; ADPE = Abiotic depletion potential for non-
fossil resources; ADPF = Abiotic depletion potential for fossil resources; WDP = Water (user) deprivation potential
RESULTS OF THE LCA - INDICATORS TO DESCRIBE RESOURCE USE according to EN 15804+A2: 1 m2
Amorim Wise Cork Pure UV
Indicator Unit A1-A3 A4 A5 B2 C1 C2 C2/1 C2/2 C3 C3/1 C4 C4/2 D D/1 D/2
PERE [MJ] 4.38E+0 3.79E-2 4.85E-2 1.49E-1 0.00E+0 3.01E-3 3.01E-3 3.01E-3 1.75E+14.39E+1 7.15E-3 1.19E-2-1.25E+1-8.90E+0-1.48E+1
PERM [MJ] 4.39E+10.00E+0-3.63E-17.16E-2 0.00E+00.00E+00.00E+00.00E+0-1.74E+1-4.35E+10.00E+00.00E+0-5.93E+0-1.48E+10.00E+0
PERT [MJ] 4.82E+1 3.79E-2-3.15E-12.21E-1 0.00E+0 3.01E-3 3.01E-3 3.01E-3 1.00E-1 4.00E-1 7.15E-3 1.19E-2-1.84E+1-2.37E+1-1.48E+1
PENRE [MJ] 9.59E+02.45E+0 2.09E-1 9.25E-1 0.00E+0 2.74E-1 2.74E-1 2.74E-1 6.92E+01.73E+1 4.28E-1 7.14E-1-2.68E+1-5.52E+1-7.93E+0
PENRM [MJ] 1.69E+10.00E+0-4.49E+01.45E+00.00E+00.00E+00.00E+00.00E+0-4.96E+0-1.24E+10.00E+00.00E+0-3.17E+0-7.93E+00.00E+0
PENRT [MJ] 2.65E+12.45E+0-4.28E+02.37E+00.00E+0 2.74E-1 2.74E-1 2.74E-1 1.96E+04.90E+0 4.28E-1 7.14E-1-3.00E+1-6.31E+1-7.93E+0
SM [kg] 0.00E+00.00E+00.00E+00.00E+00.00E+00.00E+00.00E+00.00E+00.00E+00.00E+00.00E+00.00E+0 4.57E-1 4.57E-1 4.57E-1
RSF [MJ] 0.00E+00.00E+00.00E+00.00E+00.00E+00.00E+00.00E+00.00E+00.00E+00.00E+00.00E+00.00E+00.00E+00.00E+00.00E+0
NRSF [MJ] 0.00E+00.00E+00.00E+00.00E+00.00E+00.00E+00.00E+00.00E+00.00E+00.00E+00.00E+00.00E+00.00E+00.00E+00.00E+0
FW [m³] 1.53E-1 2.40E-3 2.83E-2 1.19E-2 0.00E+0 2.04E-4 2.04E-4 2.04E-4 6.61E-4 1.65E-3 7.93E-4 1.32E-3-2.39E-1-5.03E-1-6.32E-2
PERE = Use of renewable primary energy excluding renewable primary energy resources used as raw materials; PERM = Use of
renewable primary energy resources used as raw materials; PERT = Total use of renewable primary energy resources; PENRE = Use of
non-renewable primary energy excluding non-renewable primary energy resources used as raw materials; PENRM = Use of non-
Caption
renewable primary energy resources used as raw materials; PENRT = Total use of non-renewable primary energy resources; SM = Use
of secondary material; RSF = Use of renewable secondary fuels; NRSF = Use of non-renewable secondary fuels; FW = Use of net fresh
water
RESULTS OF THE LCA – WASTE CATEGORIES AND OUTPUT FLOWS according to EN 15804+A2:
1 m2 Amorim Wise Cork Pure UV
Indicator Unit A1-A3 A4 A5 B2 C1 C2 C2/1 C2/2 C3 C3/1 C4 C4/2 D D/1 D/2
HWD [kg] 2.28E-5 1.46E-6 4.27E-6 8.61E-8 0.00E+0 1.60E-7 1.60E-7 1.60E-7 3.07E-7 7.68E-7 3.34E-7 5.56E-7-3.53E-5-7.28E-5-1.02E-5
NHWD [kg] 3.31E-1 7.67E-2 6.51E-1 4.45E-4 0.00E+0 1.30E-2 1.30E-2 1.30E-2 1.85E-2 4.62E-2 1.58E+02.63E+0-1.56E-1-2.78E-1-7.41E-2
RWD [kg] 8.71E-5 1.64E-5 1.61E-5 4.05E-7 0.00E+0 1.86E-6 1.86E-6 1.86E-6 3.31E-7 8.28E-7 2.59E-6 4.32E-6-1.89E-4-4.32E-4-2.64E-5
CRU [kg] 3.26E-1 0.00E+00.00E+00.00E+00.00E+00.00E+00.00E+00.00E+00.00E+00.00E+00.00E+00.00E+00.00E+00.00E+00.00E+0
MFR [kg] 1.31E-1 0.00E+0 4.61E-1 0.00E+00.00E+00.00E+00.00E+00.00E+00.00E+00.00E+00.00E+00.00E+00.00E+00.00E+00.00E+0
MER [kg] 4.39E+00.00E+00.00E+00.00E+00.00E+00.00E+00.00E+00.00E+00.00E+00.00E+00.00E+00.00E+0 8.68E-1 2.17E+00.00E+0
EEE [MJ] 0.00E+00.00E+00.00E+00.00E+00.00E+00.00E+00.00E+00.00E+08.72E+02.18E+10.00E+00.00E+00.00E+00.00E+00.00E+0
EET [MJ] 0.00E+00.00E+00.00E+00.00E+00.00E+00.00E+00.00E+00.00E+00.00E+00.00E+00.00E+00.00E+00.00E+00.00E+00.00E+0
HWD = Hazardous waste disposed; NHWD = Non-hazardous waste disposed; RWD = Radioactive waste disposed; CRU = Components
Caption for re-use; MFR = Materials for recycling; MER = Materials for energy recovery; EEE = Exported electrical energy; EET = Exported
thermal energy
RESULTS OF THE LCA – additional impact categories according to EN 15804+A2-optional:
1 m2 Amorim Wise Cork Pure UV
Indicator Unit A1-A3 A4 A5 B2 C1 C2 C2/1 C2/2 C3 C3/1 C4 C4/2 D D/1 D/2
[Disease
PM ND ND ND ND ND ND ND ND ND ND ND ND ND ND ND
Incidence]
[kBq U235-
IRP ND ND ND ND ND ND ND ND ND ND ND ND ND ND ND
Eq.]
ETP-fw [CTUe] ND ND ND ND ND ND ND ND ND ND ND ND ND ND ND
HTP-c [CTUh] ND ND ND ND ND ND ND ND ND ND ND ND ND ND ND
HTP-nc [CTUh] ND ND ND ND ND ND ND ND ND ND ND ND ND ND ND
SQP [-] ND ND ND ND ND ND ND ND ND ND ND ND ND ND ND
PM = Potential incidence of disease due to PM emissions; IR = Potential Human exposure efficiency relative to U235; ETP-fw = Potential
Caption comparative Toxic Unit for ecosystems; HTP-c = Potential comparative Toxic Unit for humans (cancerogenic); HTP-nc = Potential
comparative Toxic Unit for humans (not cancerogenic); SQP = Potential soil quality index
Disclaimer 1 – for the indicator IRP
This impact category deals mainly with the eventual impact of low-dose ionizing
radiation on human health of the nuclear fuel cycle. It does not consider effects due to possible
nuclear accidents, occupational exposure or radioactive waste disposal in underground
facilities. Potential ionizing radiation from the soil, radon and from some construction materials is also not
measured by this indicator.
Disclaimer 2 – for the indicators ADPE, ADPF, WDP, ETP-fw, HTP-c, HTP-nc, SQP
The results of this environmental impact indicator shall be used with care as the
uncertainties on these results are high as there is limited experience with the indicator.
6. LCA: Interpretation
This chapter contains an interpretation of the Life The high impacts of the product stage of Amorim Cork
Cycle Impact Assessment categories. When Pure UV, show the relevance of the manufacturing
expressed as a percentage, the impact refers to its processes, which are mostly related to the use of
magnitude expressed as a percentage of the total chemical products and electricity consumption, whose
product impact across all modules, with the exception production and use generate emissions of diverse
of module D. pollutants to the atmosphere and discharges of sludge
The product stage (A1-A3) of Amorim Wise Cork Pure waste and wastewater.
UV has the highest impacts for all impact categories Amorim Cork Pure UV end-of-life (mix scenario) (C1-
assessed, while the use stage (B2), considering a C4) also carries relevant potential impacts overall. The
lifetime of 1 year, has low impacts for most of the end-of-life stage presents the highest contribution for
impact categories, when compared with other stages. the Global Warming Potential (GWP) – total
category, representing 50 % of the result, followed by a
8 Environmental Product Declaration Amorim Cork Flooring – Amorim Wise Cork Pure UV
contribution of 43 % in the Global Warming Potential potential (EP) - marine impact category.
(GWP) – biogenic category, and 19% of Eutrophication
7. Requisite evidence
INDOOR AIR QUALITY
Compliance with the strictest indoor air quality
standards after being tested on over 2000 potential
chemicals.
French regulation on VOC emissions
French certification, which classifies products Results
according to their level of VOC emissions. Our Concentration limits after 3, 7 and 28 days of exposure
products have been classified at the highest level (A+). are presented in the following tables:
GREENGUARD Certification Quality Standard
Greenguard North-American certification identifies
products that have low chemical emissions, improving
the air in which they are used. Our products are
awarded the GOLD certification. A stricter certification
criteria which ensures that a product is acceptable for
use in environments such as schools and healthcare
facilities.
TÜV PROFiCERT
Tüv-Proficert is a transnational certificate for VOC-
emission and air quality, certifying that a product
complies with different national regulations such as
AgBB (Germany), Belgian VOV regulation, Finnish M1,
breeam, leed v4 (outside North America), ral -uz 120
and Austrian Ecolabel (Guideline uz 56). In October
Quality PREMIUM
2018 Amorim Cork Flooring was the first flooring
company to achieve tüv certification at its highest level
- Premium.
9 Environmental Product Declaration Amorim Cork Flooring – Amorim Wise Cork Pure UV
8. References
AgBB EN 14085
Umweltbundesamt Germany, Health-related EN 14085:2010 - Resilient floor coverings -
Evaluation of Emissions of Volatile Organic Specification for floor panels for loose laying
Compounds (VVOC, VOC and SVOC) from Building
Products
EN 15804
Austrian Ecolabel EN 15804:2012-04+A2 2019: Sustainability of
Austrian Ecolabel, Guideline uz 56, Österreichisches construction works — Environmental Product
Umweltzeichen, Stubenbastei 5, A-1010 Wien, Austria Declarations — Core rules for the product category of
construction products
BREEAM
Building Research Establishment Environmental EU/BPR
Assessment Method, Building Research Establishment Regulation (EU) 528/2012 (BPR), European
UK (BRE) Union/Biocidal Products Regulation (EU/BPR)
BS EN 12667 EU/EFTA
BS EN 12667:2001 - Thermal performance of building Regulation (EU) No. 305/2011 (CPR), European
materials and products. Determination of thermal Union/European Free Trade Association (EU/EFTA)
resistance by means of guarded hot plate and
heat flow meter methods. Products of high and Eurofins Product Testing A/S
medium thermal resistance RAL-UZ 120 - Eurofins Miljo, Smedeskowej 38, 8464
Galten, Denmark
DIN EN 717-1
DIN EN 717-1:2005 - Wood-based panels - European List of Waste
Determination of formaldehyde release - Part 1: European List of Waste (ELW) (Commission Decision
Formaldehyde emission by the chamber method 2000/532/EC)
EN 12104 European Waste Catalogue Directive
EN 12104:2018 - Resilient floor coverings - Cork floor European Waste Catalogue (EWC) (Commission
tiles – Specification Decision 94/3/EC)
EN 13329 European Waste Framework Directive
EN 13329:2000 - Laminate floor coverings. Waste Framework Directive (WFD) (2008/98/EC)
Specifications, requirements and test methods
GREENGUARD
EN 13501-1 Greenguard North-American certification
EN13501-1:2007:Fire classification of construction
products and building elements-Part1: Classification Institut Bauen und Umwelt
using data from reaction to fire tests Institut Bauen und Umwelt e.V.: General Instructions
for the EPD programme of Institut Bauen und Umwelt
EN 13893 e.V., Version 2.0, Berlin: Institut Bauen und Umwelt
EN 13893:2002 - Resilient, laminate and textile floor e.V., 2021.
coverings. Measurement of dynamic coefficient of www.ibu-epd.com
friction on dry floor surfaces
ISO 105-B02
EN 14041 ISO 105-B02:2013 - Textiles -- Tests for colour
EN 14041:2004 - Resilient, textile and laminate floor fastness -- Part B02: Colour fastness to artificial light:
coverings – Essential characteristics Xenon arc fading lamp test
10 Environmental Product Declaration Amorim Cork Flooring – Amorim Wise Cork Pure UV
ISO 10874
ISO 10874:2009 - Resilient, textile and laminate floor ISO 4918
coverings -- Classification ISO 4918:2009 - Resilient, textile and laminate floor
coverings -- Castor chair test
ISO 14025
DIN EN ISO 14025:2011-10: Environmental labels and LEED
declarations — Type III environmental declarations — LEED v4: Reference Guide for Building Design and
Principles and procedures Construction - Outside North America
ISO 16000-6 PCR Part A+A2, version 1.1.1
ISO 16000-6:2011 - Indoor air - Part 6: Determination Institut Bauen und Umwelt e.V., Berlin (pub.): Product
of volatile organic compounds in indoor and test Category Rules for Construction Products from the
chamber air by active sampling on Tenax TA sorbent, range of Environmental Product Declarations of Institut
thermal desorption and gas chromatography using MS Bauen und Umwelt (IBU), Part A: Calculation Rules for
or MS-FID the Life Cycle Assessment and Requirements on the
Project Report according to EN 15804+A2:2019. April
ISO 16000-9 2021 (www.bau-umwelt.de)
ISO 16000-9:2006 - Indoor air - Part 9: Determination
of the emission of volatile organic compounds from PCR Part B
building products and furnishing -- Emission test Product Category Rules for Construction Products
chamber method from the range of Environmental Product Declarations
of Institut Bauen und Umwelt (IBU), Part B:
ISO 16581 Requirements on the EPD for floor coverings, V1.2,
ISO 16581:2014 - Resilient and laminate floor Berlin: Institut Bauen und Umwelt e.V. (IBU), February
coverings -- Determination of the effect of simulated 2018
movement of a furniture leg
REACH
ISO 23997 Regulation (EC) No 1907/2006, Regulation concerning
ISO 23997:2007- Resilient floor coverings -- the Registration, Evaluation, Authorization and
Determination of mass per unit area Restriction of Chemicals (REACH)
ISO 24336 SimaPro
ISO 24336:2005 - Laminate floor coverings - SimaPro software-system version 9.1 (PRé
Determination of thickness swelling after partial consultants) and Ecoinvent 3.5 database, 2018
immersion in water
UL 2818 - 2013
ISO 24342 UL 2818 - 2013 Standard for Chemical Emissions for
ISO 24342:2007 - Resilient and textile floor-coverings - Building Materials, Finishes and Furnishings
- Determination of side length, edge straightness and
squareness of tiles
ISO 24343 – 1
ISO 24343-1:2007 - Resilient and laminate floor
coverings -- Determination of indentation and residual
indentation -- Part 1: Residual indentation
11 Environmental Product Declaration Amorim Cork Flooring – Amorim Wise Cork Pure UV
Publisher
Institut Bauen und Umwelt e.V. Tel +49 (0)30 3087748- 0
Panoramastr. 1 Fax +49 (0)30 3087748- 29
10178 Berlin Mail info@ibu-epd.com
Germany Web www.ibu-epd.com
Programme holder
Institut Bauen und Umwelt e.V. Tel +49 (0)30 - 3087748- 0
Panoramastr 1 Fax +49 (0)30 – 3087748 - 29
10178 Berlin Mail info@ibu-epd.com
Germany Web www.ibu-epd.com
Author of the Life Cycle
Assessment Tel +351 217 912 000
Ernst & Young Audit & Associados Fax +351 217 957 590
- SROC, SA Mail sustentabilidade@pt.ey.com
Avenida da República 90 Web http://www.ey.com
1649- 024 Lisboa
Portugal
Owner of the Declaration
Amorim Cork Flooring, S. A. Tel +351 227 475 600
Rua do Ribeirinho 202 Fax +351 227 475 601
4536-907 S. PAIO DE OLEIROS Mail geral.ar@amorim.com
Portugal Web www.amorimcorkflooring.com
