ENVIRONMENTAL PRODUCT DECLARATION
as per ISO 14025 and EN 15804+A2
Owner of the Declaration Unilin BV, division flooring
Publisher Institut Bauen und Umwelt e.V. (IBU)
Programme holder Institut Bauen und Umwelt e.V. (IBU)
Declaration number EPD-UNI-20230479-IBC1-EN
Issue date 15.01.2024
Valid to 14.01.2029
Luxury Vinyl Tiles (LVT)
Unilin BV, division flooring
www.ibu-epd.com | https://epd-online.com
1. General Information
Unilin BV, division flooring Luxury Vinyl Tiles (LVT)
Programme holder Owner of the declaration
IBU – Institut Bauen und Umwelt e.V. Unilin BV, division flooring
Hegelplatz 1 Ooigemstraat 3
10117 Berlin 8710 Wielsbeke
Germany Belgium
Declaration number Declared product / declared unit
EPD-UNI-20230479-IBC1-EN 1m² of Luxury Vinyl Tiles (LVT) floating floor (5 mm thickness without
underlay) with mechanical locking.
This declaration is based on the product category rules: Scope:
Floor coverings, 01.08.2021 In this EPD semi flexible LVT floating floor with mechanical locking
(PCR checked and approved by the SVR) according to EN 16511:2023 Modular mechanical locked floor coverings
(MMF) - Specification, requirements and test method for multilayer
modular panels for floating installation are declared.
Issue date
The results are representative of production in UNILIN B.V. Division
15.01.2024
Flooring, Avelgem site (Belgium).
This EPD covers printed laminate polyvinyl chloride floor coverings
Valid to
produced by Unilin under following brands:
14.01.2029
• Quick-Step (Alpha Vinyl, Alpha Vinyl pad, Paso Rigid Click,
Lima Rigid Click, Rigid Vinyl, Sens by Quick-Step)
• Quick-Step Howdens (Plank, Hybrid, Rigid Vinyl Pad Plank,
Rigid Vinyl Pad Tile)
• Pergo (Rigid Click Pro, Rigid click PAD Pro, Saimaa pro,
Vibrance by Pergo)
• Moduleo (Next, LAYRED)
• LOC (Tender, Tender Base)
• Vitality (Amuse, Amuse base)
• Elka (Rigid, Rigid Pad)
• Unilin (Vinyl Rigid, Vinyl Rigid Pad)
• ORIGIN (30 & 55)
Dipl.-Ing. Hans Peters • Engineered click acoustic
(Chairman of Institut Bauen und Umwelt e.V.) • Textura acoustic
The owner of the declaration shall be liable for the underlying information
and evidence; the IBU shall not be liable with respect to manufacturer
information, life cycle assessment data and evidences.
The EPD was created according to the specifications of EN 15804+A2. In
the following, the standard will be simplified as EN 15804.
Verification
The standard EN 15804 serves as the core PCR
Independent verification of the declaration and data according to ISO
14025:2011
internally X externally
Florian Pronold Dr. Frank Werner,
(Managing Director Institut Bauen und Umwelt e.V.) (Independent verifier)
1 Environmental Product Declaration - Unilin BV, division flooring - Luxury Vinyl Tiles (LVT)
2. Product
• Voluntary data: The product complies with the
2.1 Product description/Product definition requirements of the following standard, too EN
Rigid vinyl floorings also called Luxury Vinyl Tiles (LVT) are 16511:2023 Modular mechanical locked floor coverings
made up of several layers. On the top side, there is a PVC (MMF) - Specification, requirements and test method for
decor layer (2) with a transparent PVC wear-resistant contact multilayer modular panels for floating installation. For
surface coated with a PU lacquer for a mat aspect with an the application and use the respective national
excellent stain and friction resistance (1); in the middle, for provisions apply.
extra acoustic and walking comfort an additional soft PVC layer
(3) and on the back side, there is a core layer (4) made of 2 2.4 Delivery status
rigid PVC layers reinforced with unwoven glass- fibers and LVT floor covering is delivered in planks or tiles.
separated by a foamed PVC layer for acoustic and comfort Typical standard dimensions are as follows (length - width
reasons to guarantee floor stability and to avoid telegraphing thickness)
effect from subfloor irregularities. Some references are
• 1251mm x 189mm x 5mm (4+1mm)
produced with a 1mm pre-attached underlay to make the
• 610mm x 303mm x 5mm (4+1mm)
installation faster and easier. The decorative PVC layer of LVT
• 630mm x 126mm x 6mm (5+1mm)
floor covering can be printed with any design and gives the
• 1494mm x 209mm x 6mm (5+1mm)
floor its individual appearance. The planks have a mechanical
• 856mm x 428mm x 6mm (5+1mm)
and patented connection (Uniclic, Unidrop, Unizip).
• 630mm x 126mm x 6mm (5+1mm)
• 1253mm x 189mm x 6mm (5+1mm)
• 1317mm x 189mm x 6mm (5+1mm)
• 610mm x 303mm x 6mm (5+1mm)
• 1251mm x 189mm x 4mm
• 610mm x 303mm x 4mm
2.5 Base materials/Ancillary materials
The product group has the following composition:
• Filler 51%
• Polymers (PVC) 36%
• Plasticizer and stabilizer 8%
• Other 5%
This product contains substances listed in the Candidate List of
Substances of Very High Concern for Authorisation REACH
(date: 16.11.2023) exceeding 0.1 percentage by mass: NO
This product contains other CMR substances in categories 1A
or 1B which are not on the candidate list, exceeding 0.1
For the placing on the market of the product in the European
percentage by mass: NO
Union/European Free Trade Association (EU/EFTA) (with the
exception of Switzerland) Regulation (EU) No. 305/2011 (CPR)
Biocide products were added to this construction product or it
applies. The product needs a declaration of performance taking
has been treated with biocide products (this then concerns a
into consideration EN 14041:2004 AC 2006 Resilient, textile
treated product as defined by the (EU) Ordinance on Biocide
and laminate floor coverings - Essential characteristics and the
Products No. 528/2012): NO
CE-marking.
For the application and use the respective national provisions
2.6 Manufacture
apply.
The material efficiency is 99% as all production waste are
internally recycled as raw material.
2.2 Application In production a certified ISO 9001 quality control system is in
place.
According to EN ISO 10874 the area of application for resilient
floor coverings is indicated by use classes. The declared
2.7 Environment and health during manufacturing
product group covers the use classes between 32 and 33.
The production conditions do not demand any special health
2.3 Technical Data protection measures over and beyond the legal requirements.
Water
Constructional data
Production is using river water for cooling. The use of
Name Value Unit water in the LVT flooring production process is negligible.
Product minimum thickness 4 mm Where water is needed, it is re-used in the
internal water loop and eventually reinjected in the river after
Product maximum thickness 5+1 mm
controlling quality and temperature.
Product minimum mass 6.7 kg/m²
Air
Product maximum mass 8.7 kg/m²
The constitutional valid regulations are observed. The
Product form Planks and Tiles emissions to air are far below the legally required thresholds.
Soil
• Performance data of the product in accordance with the
There is no impact on soil.
declaration of performance with respect to its essential
characteristics according to EN 14041:2004 AC 2006
In production a certified ISO 14001 environmental management
Resilient, textile and laminate floor coverings - Essential
system is in place.
characteristics and the CE marking.
2 Environmental Product Declaration - Unilin BV, division flooring - Luxury Vinyl Tiles (LVT)
the flooring will most probably be OK as no visible damage are
2.8 Product processing/Installation expected.
UNILIN LVT click floor coverings are generally installed floating. If the water came under the floorcovering (floating installation) it
This means that the floor covering is not fixed to the sub-floor may be necessary to unclick the panels and let dry the subfloor
using glue, nails etc. The floor covering panels are mainly and the underlay. It should be given the time to come to
mechanically assembled glue-less by means of tongue and equilibrium moisture content before reinstallation of the dried
groove. Underlay material is needed when installing LVT click panels.
floor coverings in order to achieve a leveling effect, thermal or Most of the LVT ranges offer a special watertightness between
acoustical insulation. planks/tiles. During the installation, the periphery needs to be
treated with a foam strip and a special sealant to avoid
2.9 Packaging
infiltration. In case of water spillage on the surface, it will
LVT tiles are packed together. The packs are protected using evaporate before having the chance to penetrate between
cardboard 6-sided boxes. The packaging cardoard is fully planks/tiles.
recyclable.
The packs are palletized on wooden pallets using wood from Mechanical destruction
controlled origin. The pallets can be re-used (Euro pallets) or Small damages in the flooring surface can be repaired by using
recycled as wood category 03 01 05 according to the European colored solvent-free melt waxes. Scratches in the transparent
Waste Catalogue. wear layer can be repaired with an adapted new coating 1 or 2
compound following the manufacturer instructions. In case of
2.10 Condition of use
more severe damage the damaged panels can be replaced.
A Polyurethan-based lacquer is used for the production of the
Procedures to repair or replace a damaged plank are available
flooring panels. After exposure to a strong UV light under
on request. The damaged panels go into the normal end-of-life
anaerobicconditions, this coating is 3D crosslinked by an
treatment.
irreversible reaction andcompletely closing the flooring surface.
Under normal conditions, the coatingis chemically stable and 2.14 Re-use phase
mechanically firmly bonded to the PVC wearlayer. A LVT click floor covering which is not at the end-of-life stage
may be un-installed and re-used as a floor covering. Post-
2.11 Environment and health during use
consumer LVT click floor covering waste can be recycled as
Environmental protection
PVC-based products. When appropriate recycling facilities do
When the products are used as designated and according the
not exist, LVT click floor coverings shall be thermally valorized.
current state of knowledge, there are no hazards for water, air
and soil. 2.15 Disposal
Health protection Post-installation and post-consumer flooring panels are
When used normally and in accordance with the designated considered as PVC waste. The European Waste Code EWC is
purpose, no health risks or restrictions are to be anticipated by 070213. It can be disposed in any regulated municipal waste
UNILIN LVT floor coverings. This is in line with the current state collection point in the combustible waste container. Unilin offers
of knowledge. a take-back program named Recover to enable circularity of
PVC flooring. Please contact your local Unilin dealer to check
2.12 Reference service life
the availability of this Recover program in your country.
The BBSR gives a general useful life of 20 years for floor
coverings of component group 352.711. Due to the 2.16 Further information
comparatively high resistance of the LVT floorings, Unilin grants All information about the product composition, technical
an additional warranty (based on the floor owner life according performance, instructions for installation and maintenance,
to the manufacturer's warranty conditions) for the declared precautionary instructions for use, CE marking and relevant
product. In order to increase the life duration of the floor DOP (declaration of performance) documents, are available
covering, the manufacturer's instructions concerning warranty either in the packs or can be found on the homepage
and care must be observed, available for download at www.unilin.com/en/flooring or can be requested at Unilin BV
www.unilin.com/en/flooring. The use stage is declared in this division flooring info@unilin.com.
EPD for a one year usage.
2.13 Extraordinary effects
Fire
The reaction to fire is determined according to EN 13501-1. The
class for LVT floors produced by UNILIN BV division Flooring,
in combination with all underlays of the sales program is Bfl-s1.
Fire protection
Name Value
Building material class Bfl
Smoke gas development s1
Water
In case of a leak or a flood where the flooring has been soaked
3. LCA: Calculation rules
1m² of Luxury Vinyl Tiles (LVT) floating floor (5 mm thickness
3.1 Declared Unit without underlay) with mechanical locking.
3 Environmental Product Declaration - Unilin BV, division flooring - Luxury Vinyl Tiles (LVT)
Declared unit and mass reference In the assessment, all available data from the production
process are considered, i.e. all raw materials used, utilised
Name Value Unit
thermal energy, and electric power consumption using best
Declared unit 1 m2 available LCI datasets. Thus material and energy flows
Layer thickness 0.005 m contributing less than 1% of mass or energy are also
Grammage 8.6 kg/m2 considered.
No flows were cut-off that are known to have significant
3.2 System boundary
environmental impacts.
Type of EPD according to EN 15804: cradle to grave.
3.5 Background data
Modules A1-A3 include processes that provide materials and Used background data comes from ecoinvent database version
energy input for the system, manufacturing and transport 3.8 from 2021. It has been selected to be representative of
processes up to the factory gate, as well as waste processing. processes geographic location.
Module A4 includes transport of the floor covering to the place 3.6 Data quality
of installation. A4 data are based on a weighted average Primary data refer to the year 2021. The data of the foreground
distance for worldwide deliveries. processes is based on input-output analyses at the Belgian
production sites. The primary data collection was done
Module A5 includes the production of offcuts for the installation thoroughly, all relevant flows were considered.
of the floor covering, and incineration of offcuts and packaging
material. 3.7 Period under review
The period under review for primary data is 2021.
Module B2 is including provision of cleaning agent, energy and
3.8 Geographic Representativeness
water consumption for the cleaning of the floor covering. The
LCA results in this EPD are declared for a one-year usage. Land or region, in which the declared product system is
manufactured, used or handled at the end of the product´s
Module C2 includes transportation of the postconsumer waste lifespan: Global
to waste processing.
3.9 Allocation
End of life scenarios are declared for:
The overall production of UNILIN comprises further products
• 100% landfilling (Scenario 1, C4/1)
beside the product considered in this study. Data for thermal
• 100% incineration in a waste incineration plant (WIP)
and electrical energy as well as auxiliary material refer to the
(Scenario 2, C4/2)
declared product. During data collection the allocation is done
Module D includes potential benefits from all net flows given in
via mass (kg). Specific information on allocation within the
module A5 and C4 that leave the product boundary system
background data is given in the ecoinvent documentation.
after having passed the end-of-waste state in the form of
recovery and/or recycling potentials. Module D is declared for 3.10 Comparability
each scenario separately (D/1 and D/2). Basically, a comparison or an evaluation of EPD data is only
possible if all the data sets to be compared were created
3.3 Estimates and assumptions
according to EN 15804 and the building context, respectively
No additional estimates or assumptions had to be made
the product-specific characteristics of performance, are taken
beyond the information stated in clauses 3 and 4.
into account.
Background database is as described in chapter 3.5.
3.4 Cut-off criteria
4. LCA: Scenarios and additional technical information
Name ValueUnit
Characteristic product properties of biogenic carbon
Transport distance by truck 686 km
Information on describing the biogenic carbon content at Capacity utilisation (including empty runs) by truck 67 %
factory gate
transport distance by boat 1319 km
Name ValueUnit
kg Installation in the building (A5)
Biogenic carbon content in product -
C Name Value Unit
Biogenic carbon content in accompanying kg Product installation losses 4.0 %
0.3
packaging C Product packaging waste 0.66 kg
Note: 1 kg of biogenic carbon is equivalent to 44/12 kg of CO .
2
The following technical information is a basis for the declared
Maintenance (B2)
modules. Scenarios correspond to the worldwide production
Maintenance scenario is:
and consumption.
• 1 vacuum cleaning per week,
Transport to the construction site (A4)
• 1 wet cleaning (water and detergent) per month.
Product shipping stage A4 represents weighted average based
on worldwide sales.
4 Environmental Product Declaration - Unilin BV, division flooring - Luxury Vinyl Tiles (LVT)
Name Value Unit End of Life (C1-C4)
Water consumption 1.33 kg/m²/year
Name Value Unit
Detergent 0.0133 kg/m²/year
Energy recovery from waste (for EoL scenario 2) 8.6 kg
Electricity consumption (European mix) 0.54 kWh/m²/year
Landfilling (for EoL scenario 1) 8.6 kg
Energy recovery from product waste is assumed in a municipal
Reference service life waste incineration plant with energy efficiency < 60%. In line
with EN 15804, this is therefore declared as part of module C4.
Name Value Unit
Reference service life according to BBSR 20 a
5 Environmental Product Declaration - Unilin BV, division flooring - Luxury Vinyl Tiles (LVT)
5. LCA: Results
The results refer to LVT thickness of 5 mm without underlay (8.6 kg/m²). The information on maintenance is declared per year.
LVT floor coverings are available in thicknesses 4 mm and 5mm, with and without underlay. In order to enable the user of the EPD to
calculate the results for different thicknesses and use classes the factors in the following table can be used for the calculation. For A1,
A2, A3, A4, A5, B2, C4 and D the LCA results of the declared product (thickness 5 mm without underlay) in following tables have to be
multiplied with these factors.
6 Environmental Product Declaration - Unilin BV, division flooring - Luxury Vinyl Tiles (LVT)
DESCRIPTION OF THE SYSTEM BOUNDARY (X = INCLUDED IN LCA; MND = MODULE OR INDICATOR NOT DECLARED; MNR
= MODULE NOT RELEVANT)
Benefits and
Construction loads beyond
Product stage Use stage End of life stage
process stage the system
boundaries
la ire ta m w a Ry lp p u s tro p s n a rT g n iru tc a fu n a M e h t m o rf tro p s n a rTe tis e h t o t e ta g y lb m e s s A e s U e c n a n e tn ia M ria p e R tn e m e c a lp e R tn e m h s ib ru fe R y g re n e la n o ita re p Oe s u re ta w la n o ita re p Oe s u n o itc u rts n o c -e Dn o itilo m e d tro p s n a rT g n is s e c o rp e ts a W la s o p s iD -e s u e R-y re v o c e R-g n ilc y c e Rla itn e to p
A1 A2 A3 A4 A5 B1 B2 B3 B4 B5 B6 B7 C1 C2 C3 C4 D
X X X X X MND X MNR MNR MNR MND MND X X X X X
RESULTS OF THE LCA - ENVIRONMENTAL IMPACT according to EN 15804+A2: 1 m² LVT floor covering
Parameter Unit A1 A2 A3 A4 A5 B2 C1 C2 C3 C4/1 C4/2 D/1 D/2
GWP-total kg CO 2 eq 9.99E+00 1.5E-01 4.7E+00 1.14E+00 2.25E+00 2.34E-01 0 3.72E-02 0 6.01E-01 1.09E+01 -4.87E-02 -2.87E+00
GWP-fossil kg CO 2 eq 9.91E+00 1.5E-01 5.53E+00 1.14E+00 1.17E+00 2.29E-01 0 3.72E-02 0 6.01E-01 1.09E+01 -4.82E-02 -2.86E+00
GWP-
biogenic kg CO 2 eq -8.21E-02 4.88E-05 -8.36E-01 3.48E-04 1.07E+00 1.21E-03 0 1.21E-05 0 8.78E-05 3.11E-03 -4.92E-04 -6.52E-03
GWP-luluc kg CO 2 eq 1.54E-01 5.81E-05 1.39E-02 5.04E-04 6.76E-03 3.98E-03 0 1.44E-05 0 1.88E-05 7.9E-04 -4.37E-05 -2.86E-03
kg CFC11
ODP 3.27E-06 3.78E-08 7.67E-07 2.63E-07 1.91E-07 1.24E-08 0 9.35E-09 0 2.67E-08 2.96E-07 -4.76E-09 -3.14E-07
eq
AP mol H+ eq 4.92E-02 4.83E-04 1.39E-02 6.69E-03 3.27E-03 1.32E-03 0 1.19E-04 0 6.39E-04 5.43E-03 -1.44E-04 -7.84E-03
EP-
kg P eq 4.07E-04 1.08E-06 1.32E-04 7.81E-06 2.32E-05 2.5E-05 0 2.67E-07 0 6.2E-07 2.53E-05 -2.14E-06 -1.29E-04
freshwater
EP-marine kg N eq 8.89E-03 1.06E-04 3.5E-03 1.51E-03 7.13E-04 2.23E-04 0 2.63E-05 0 4.11E-04 1.36E-03 -2.36E-05 -1.24E-03
EP-terrestrial mol N eq 9E-02 1.18E-03 3.28E-02 1.68E-02 7.27E-03 2.03E-03 0 2.92E-04 0 2.58E-03 1.46E-02 -2.65E-04 -1.4E-02
kg NMVOC
POCP 3.67E-02 4.65E-04 9.48E-03 5.16E-03 2.51E-03 5.46E-04 0 1.15E-04 0 8.87E-04 4.16E-03 -8.5E-05 -4.16E-03
eq
ADPE kg Sb eq 3.46E-04 3.74E-07 3.87E-05 3.93E-06 1.61E-05 2.3E-06 0 9.26E-08 0 2.52E-07 1.16E-05 -7.37E-08 -3.1E-06
ADPF MJ 2.51E+02 2.47E+00 1.09E+02 1.72E+01 1.6E+01 4.82E+00 0 6.1E-01 0 1.93E+00 1.25E+01 -9.05E-01 -5.44E+01
m3 world
WDP eq 1.32E+01 8.48E-03 2.11E+00 5.04E-02 6.79E-01 7.05E-02 0 2.1E-03 0 9.25E-03 8.7E-01 -6.05E-03 -2.91E-01
deprived
GWP = Global warming potential; ODP = Depletion potential of the stratospheric ozone layer; AP = Acidification potential of land and water; EP =
Eutrophication potential; POCP = Formation potential of tropospheric ozone photochemical oxidants; ADPE = Abiotic depletion potential for non-fossil
resources; ADPF = Abiotic depletion potential for fossil resources; WDP = Water (user) deprivation potential)
RESULTS OF THE LCA - INDICATORS TO DESCRIBE RESOURCE USE according to EN 15804+A2: 1 m² LVT floor covering
Parameter Unit A1 A2 A3 A4 A5 B2 C1 C2 C3 C4/1 C4/2 D/1 D/2
PERE MJ 1.5E+01 3.14E-02 1.16E+01 2.35E-01 2.35E+00 1.04E+00 0 7.76E-03 0 8.38E-02 1.58E+00 2.28E-02 -4.34E+00
PERM MJ 1.01E+00 0 2.63E-01 0 -1.16E+00 8.77E-04 0 0 0 0 0 0 0
PERT MJ 1.61E+01 3.14E-02 1.18E+01 2.35E-01 1.2E+00 1.04E+00 0 7.76E-03 0 8.38E-02 1.58E+00 2.28E-02 -4.34E+00
PENRE MJ 1.44E+02 2.47E+00 1.08E+02 1.72E+01 1.65E+01 4.46E+00 0 6.1E-01 0 1.93E+00 1.19E+02 -9.05E-01 -5.44E+01
PENRM MJ 1.07E+02 0 3.7E-01 0 -4.76E-01 3.64E-01 0 0 0 0 -1.07E+02 0 0
PENRT MJ 2.51E+02 2.47E+00 1.09E+02 1.72E+01 1.6E+01 4.82E+00 0 6.1E-01 0 1.93E+00 1.25E+01 -9.05E-01 -5.44E+01
SM kg 0 0 4.88E-01 0 1.95E-02 3.28E-04 0 0 0 0 0 0 0
RSF MJ 0 0 0 0 0 0 0 0 0 0 0 0 0
NRSF MJ 0 0 0 0 0 0 0 0 0 0 0 0 0
FW m3 2.18E-01 2.87E-04 6.23E-02 1.83E-03 2.32E-02 4.34E-03 0 7.11E-05 0 2.44E-03 2.78E-01 -3.59E-04 -2.16E-02
PERE = Use of renewable primary energy excluding renewable primary energy resources used as raw materials; PERM = Use of renewable primary
energy resources used as raw materials; PERT = Total use of renewable primary energy resources; PENRE = Use of non-renewable primary energy
excluding non-renewable primary energy resources used as raw materials; PENRM = Use of non-renewable primary energy resources used as raw
materials; PENRT = Total use of non-renewable primary energy resources; SM = Use of secondary material; RSF = Use of renewable secondary fuels;
NRSF = Use of non-renewable secondary fuels; FW = Use of net fresh water
RESULTS OF THE LCA – WASTE CATEGORIES AND OUTPUT FLOWS according to EN 15804+A2:
1 m² LVT floor covering
Parameter Unit A1 A2 A3 A4 A5 B2 C1 C2 C3 C4/1 C4/2 D/1 D/2
HWD kg 4.32E-01 1.71E-03 6.32E-01 1.3E-02 1.45E-01 6.23E-03 0 4.22E-04 0 2.22E-03 2.17E+00 -5.8E-04 -2.83E-02
NHWD kg 6.65E+00 2.43E-01 1.37E+00 9.24E-01 4.07E-01 9.07E-02 0 6.01E-02 0 8.64E+00 4.86E-01 -6.16E-03 -3.56E-01
RWD kg 5.29E-04 1.67E-05 8.48E-04 1.16E-04 6.49E-05 3.41E-05 0 4.13E-06 0 1.25E-05 6.72E-05 -2.23E-06 -2.02E-04
CRU kg 0 0 0 0 0 0 0 0 0 0 0 0 0
MFR kg 0 0 1.1E-01 0 4.42E-03 4.25E-04 0 0 0 0 0 0 0
MER kg 0 0 0 0 0 0 0 0 0 0 0 0 0
7 Environmental Product Declaration - Unilin BV, division flooring - Luxury Vinyl Tiles (LVT)
EEE MJ 0 0 6.71E-01 0 1.48E+00 1.48E-03 0 0 0 0 1.07E+01 0 0
EET MJ 0 0 1.48E+00 0 2.99E+00 2.86E-03 0 0 0 0 2.37E+01 0 0
HWD = Hazardous waste disposed; NHWD = Non-hazardous waste disposed; RWD = Radioactive waste disposed; CRU = Components for re-use;
MFR = Materials for recycling; MER = Materials for energy recovery; EEE = Exported electrical energy; EET = Exported thermal energy
RESULTS OF THE LCA – additional impact categories according to EN 15804+A2-optional:
1 m² LVT floor covering
Parameter Unit A1 A2 A3 A4 A5 B2 C1 C2 C3 C4/1 C4/2 D/1 D/2
Disease
PM 3.95E-07 1.76E-08 1.27E-07 8.69E-08 2.93E-08 4.46E-09 0 4.34E-09 0 1.39E-08 3.92E-08 -3.39E-10 -2.11E-08
incidence
kBq U235
IR 5.46E-01 1.07E-02 9.78E-01 7.46E-02 6.8E-02 4.11E-02 0 2.65E-03 0 8.85E-03 6.04E-02 -3.05E-03 -2.35E-01
eq
ETP-fw CTUe 9.22E+01 8.17E-01 8.1E+01 5.91E+00 2.99E+01 8.82E-01 0 2.02E-01 0 3.21E+01 5.41E+02 -6.55E-02 -3.53E+00
HTP-c CTUh 8.01E-09 5.25E-11 2.83E-09 4.66E-10 5.99E-10 1.12E-10 0 1.3E-11 0 6.02E-11 1.49E-09 -6.09E-12 -4.81E-10
HTP-nc CTUh 1.95E-07 1.68E-09 3.88E-08 1.05E-08 1.38E-08 3.04E-09 0 4.15E-10 0 1.45E-09 4.67E-08 -1.92E-10 -1.1E-08
SQP SQP 4.72E+01 2.82E+00 6.26E+01 1.12E+01 5.39E+00 1.13E+00 0 6.98E-01 0 5.02E+00 6.07E+00 4.4E-01 -3.57E+00
PM = Potential incidence of disease due to PM emissions; IR = Potential Human exposure efficiency relative to U235; ETP-fw = Potential comparative
Toxic Unit for ecosystems; HTP-c = Potential comparative Toxic Unit for humans (cancerogenic); HTP-nc = Potential comparative Toxic Unit for humans
(not cancerogenic); SQP = Potential soil quality index
Disclaimer 1 – for the indicator “Potential Human exposure efficiency relative to U235”. This impact category deals mainly with the
eventual impact of low-dose ionizing radiation on human health of the nuclear fuel cycle. It does not consider effects due to possible
nuclear accidents, occupational exposure or radioactive waste disposal in underground facilities. Potential ionizing radiation from the
soil, radon and from some construction materials is also not measured by this indicator.
Disclaimer 2 – for the indicators “abiotic depletion potential for non-fossil resources”, “abiotic depletion potential for fossil resources”,
“water (user) deprivation potential, deprivation-weighted water consumption”, “potential comparative toxic unit for ecosystems”,
“potential comparative toxic unit for humans – cancerogenic”, “Potential comparative toxic unit for humans - not cancerogenic”,
“potential soil quality index”. The results of this environmental impact indicator shall be used with care as the uncertainties on these
results are high as there is limited experience with the indicator.
6. LCA: Interpretation
Figure : Indicator results of LVT floor covering over its life Figure : Indicator results of LVT floor covering over its life
cycle (landfilling end-of-life) cycle (incineration end-of-life)
The largest part of environmental impacts is caused during All the other modules related to the product life cycle are not
production significant.
(modules A1-A3) and at waste processing for incineration end-
of-life (module C4); comparably small impacts are caused For incineration end-of-life, benefits and burdens beyond the
during the transport of the product to the construction site. system boundary (module D) is about 5 to 15% of the impacts
over the product life cycle (modules A-C) and relate to the
Maintenance (module B2) is energy recovery from waste processing in a waste incineration
presented for 1 year of product use, so its impact can be plant that is considered to substitute natural gas (heat) and
significant over the reference service life depending on the electricity grid mix.
considered indicator.
8 Environmental Product Declaration - Unilin BV, division flooring - Luxury Vinyl Tiles (LVT)
7. Requisite evidence
7.1 formaldehyde emissions 7.2 VOC emissions on 5+1mm rigid LVT flooring
Determination of the formaldehyde emissions of a rigid LVT Determination of the VOC emissions of a LVT flooring
flooring according to according to EN 16516 and evaluation according to according to EN 16516 and evaluation according
according to different labels. – EPH Laboratory Chemical to different labels. – Eurofins Product Testing A/S –
Testing – Zellescher Weg 24 – 01217 Dresden – Germany. - Smedeskovvej 38 – 8464 Galten - Denmark. - Test Report nr
Test Report nr 2522498/3 on 'Unilin Vinyl Rigid 5 mm CL33'. 392-2020-00452501_A_EN from November 24th 2020 on
Name Value Unit 'Layred 55'.
Formaldehyde CAS nr 50-00-0 < 5 µg/m3 • Compliant with AgBB-Scheme 2018 and 2019
• Compliant with the French VOC-Regulation: A+
7.2 VOC emissions on 5mm rigid LVT flooring
Determination of the VOC emissions of a rigid LVT flooring VOC EMISSION RESULTS (AgBB) AFTER 3 DAYS
according to EN 16516 and evaluation according to different
labels. – EPH Laboratory Chemical Testing – Zellescher Weg Name Value Unit
24 – 01217 Dresden – Germany. - Test Report nr 2522498/3 on TVOC 5,7 µg/m3
'Unilin Vinyl Rigid 5 mm CL33'.
R (dimensionless) 0,082
• Compliant with AgBB-Scheme 2018 and 2021 VOC wihout LCI < 5 µg/m3
• Compliant with M1 Emission Classification of Building
Carcinogens < 1 µg/m3
Materials (Testing protocol 15.11.2017)
• Compliant with the French VOC-Regulation: A+ VOC EMISSION RESULTS (AgBB) AFTER 28 DAYS
VOC EMISSION RESULTS (AgBB) AFTER 3 DAYS Name Value Unit
TVOC < 5 µg/m3
Measurements are not available.
R (dimensionless) 0,000
VOC EMISSION RESULTS (AgBB) AFTER 28 DAYS
VOC without LCI < 5 µg/m3
Name Value Unit
Carcinogens <3 µg/m3
TVOC < 5 µg/m3
R (dimensionless) 0
VOC without LCI < 5 µg/m3
Carcinogens < 1 µg/m3
8. References
IBU 2021 formaldehyde and other carbonyl compounds in indoor air and
Institut Bauen und Umwelt e.V.: General Instructions for the test chamber air – Active sampling method.
EPD programme of Institut Bauen und Umwelt e.V., Version
2.0, Berlin: Institut Bauen und Umwelt e.V., 2021 www.ibu- ISO 16000-6:2011
epd.com ISO 16000-6:2011 – Indoor air – part 6: Determination of
volatile organic compounds in indoor and test chamber air by
EN 15804 active sampling on Tenax A sorbent, thermal desorption an gas
EN 15804:2012+A2:2019+AC:2021, Sustainability of chromatography using MS of MS-FID
construction works — Environmental Product Declarations —
Core rules for the product category of construction products. ISO 16000-9:2006
ISO 16000-9:20006 – Indoor air – part 9:
EN ISO 14044 Determination of the emissions of volatile organic compounds
Environmental management - Life cycle assessment - from building products and furnishing – Emission test chamber
Requirements and guidelines (ISO 14044:2006); German and method.
English version EN ISO 14044
EN 16511:2023
ISO 14025 Modular mechanical locked floor coverings (MMF) -
EN ISO 14025:2011, Environmental labels and declarations — Specification, requirements and test method for multilayer
Type III environmental declarations — Principles and modular panels for floating installation
procedures.
EN 14041:2004 AC 2006
ISO 14040 Resilient, textile, laminate and modular multilayer floor
ISO 14040:2006, Environmental management - Life cycle coverings - Essential characteristics
assessment - Principles and framework (ISO 14040); German
and English version EN ISO 14040 EN ISO 10874:
Resilient, textile and laminate floor coverings -- Classification
CEN/TR 15941
Sustainability of construction works - Environmental product BBSR:
declarations - Methodology for selection and use of generic Bundesinsitut für Bau-, Stadt- und Raumforschung.
data; German version CEN/TR 15941
EWC-94/3/EC
ISO 16000-3:2011 Commission Decision of 20 December 1993 establishing a list
ISO 16000-3:2011 – Indoor air – part3: Determination of of wastes pursuant to Article 1a of Counsil Directive
9 Environmental Product Declaration - Unilin BV, division flooring - Luxury Vinyl Tiles (LVT)
74/442/EEC on waste, 1993 - European Waste Catalogue and
Hazardous Waste List valid from 1 January 2002. PCR Guidance – Texts for Building-Related Products and
Services – Part B: Requirements on the EPD for floor
ecoinvent coverings - IBU Published v6 dated 19.10.2023
ecoinvent, Allocation, cut-off by classification, ecoinvent
database version 3.8 (2021)
10 Environmental Product Declaration - Unilin BV, division flooring - Luxury Vinyl Tiles (LVT)
Publisher
Institut Bauen und Umwelt e.V. +49 (0)30 3087748- 0
Hegelplatz 1 info@ibu-epd.com
10117 Berlin www.ibu-epd.com
Germany
Programme holder
Institut Bauen und Umwelt e.V. +49 (0)30 3087748- 0
Hegelplatz 1 info@ibu-epd.com
10117 Berlin www.ibu-epd.com
Germany
Author of the Life Cycle Assessment
EVEA +33 2 28 07 87 00
rue Arthur III, 11 contact@evea-conseil.com
44200 Nantes www.evea-conseil.com/en
France
Owner of the Declaration
Unilin BV, division flooring +32 56 67 52 11
Ooigemstraat 3 info@unilin.com
8710 Wielsbeke www.unilin.com/en/flooring
Belgium
11 Environmental Product Declaration - Unilin BV, division flooring - Luxury Vinyl Tiles (LVT)
