ENVIRONMENTAL PRODUCT DECLARATION
as per ISO 14025 and EN 15804+A2
Owner of the Declaration Grundfos Holding A/S
Publisher Institut Bauen und Umwelt e.V. (IBU)
Programme holder Institut Bauen und Umwelt e.V. (IBU)
Declaration number EPD-GRU-20240021-CCD2-EN
Issue date 05.06.2024
Valid to 04.06.2029
ALPHA2, ALPHA1, ALPHA2 L, ALPHA1.1, ALPHA2.1, ALPHA2.2
(Cast Iron)
Grundfos Holding A/S
www.ibu-epd.com | https://epd-online.com
General Information
Grundfos Holding A/S ALPHA2, ALPHA1, ALPHA2 L, ALPHA1.1,
ALPHA2.1, ALPHA2.2 (Cast Iron)
Programme holder Owner of the declaration
IBU – Institut Bauen und Umwelt e.V. Grundfos Holding A/S
Hegelplatz 1 Poul Due Jensens Vej 7
10117 Berlin 8850 Bjerringbro
Germany Denmark
Declaration number Declared product / declared unit
EPD-GRU-20240021-CCD2-EN 1 piece of Alpha 2/3 pump cast iron.
This declaration is based on the product category rules: Scope:
Pumps for liquids and liquids with solids, 01.08.2021 The declared product is 1 piece of ALPHA Cast Iron pump. The product is
(PCR checked and approved by the SVR) assembled in Bjerringbro, Denmark, and the life cycle assessment is
based on data collected at the production site and from supplier up- and
downstream of the supply chain. The declaration is for the variations 15-
Issue date 130, 25-130, 25-180 and 32-180, and 15-130, 25-130, 25-180 and GGES3
respectively.
05.06.2024
The owner of the declaration shall be liable for the underlying information
and evidence; the IBU shall not be liable with respect to manufacturer
Valid to
information, life cycle assessment data and evidences.
04.06.2029
The EPD was created according to the specifications of EN 15804+A2. In
the following, the standard will be simplified as EN 15804.
Verification
The standard EN 15804 serves as the core PCR
Independent verification of the declaration and data according to ISO
14025:2011
internally X externally
Dipl.-Ing. Hans Peters
(Chairman of Institut Bauen und Umwelt e.V.)
Florian Pronold Mrs Kim Allbury,
(Managing Director Institut Bauen und Umwelt e.V.) (Independent verifier)
1 Environmental Product Declaration - Grundfos Holding A/S - ALPHA2, ALPHA1, ALPHA2 L, ALPHA1.1, ALPHA2.1, ALPHA2.2 (Cast Iron)
Product
Name Value Unit
Product description/Product definition
Frequency 50 Hz
This EPD includes the cast iron ALPHA pumps. They are
Voltage 230 V
produced in different models and each new models adds a
variant expressed with an additional letter. This EPD represents Pumped liquid (e.g. water) Water -
a weighted average product that includes the data for the energy efficiency class 0.15 -
following models: Head max. Gr 1 4 m
- ALPHA2 model B-E, and the modules that follow
Head max. Gr 2 6 m
- ALPHA1 Model B, and the modules that follow
Head max. Gr 3 8 m
- ALPHA2 L Model C, and the modules that follow
- ALPHA1.1 Model B, and the modules that follow Flow range Gr 1 0 - 2.6 m3h
- ALPHA2.1 model B-E, and the modules that follow Flow range Gr 2 0 - 3.5 m3h
0 -
The size of the pump housing distinguishes the different Flow range Gr 3 m3h
2.14
pumps. The production process and production location is the
Power input Gr 1 Average (from load profile
same for all pump modules. 0.0091 kW
describing use)
For the placing on the market in the European Union/European Power input Gr 2 Average (from load profile 0.015 kW
Free Trade Association (EU/EFTA) (with the exception of describing use)
Switzerland) the following legal provisions apply: Power input Gr 3 Average (from load profile
0.023 kW
describing use)
Low Voltage Directive (2014/35/EU) Max. input power Gr 1 0.018 kW
Standards used: EN 60335-
Max. input power Gr 2 0.034 kW
1:2012+AC:2014+A11:2014+A13:2017+A1:2019+A2:2019+A15:2021,
Max. input power Gr 3 0.05 kW
EN 60335-2-51:2003+A1:2008+A2:2012.
Performance data of the product according to the harmonised
standards, based on provisions for harmonization.
EMC Directive (2014/30/EU)
Base materials/Ancillary materials
Standards used: EN 55014-1:2017, EN 55014-2:2015, EN IEC
61000-3-2:2019, EN 61000-3-3:2013. Name Value Unit
Steel and stainless steel 17.8 %
Plastic 1.3 %
Ecodesign Directive (2009/125/EC)
Plastic packaging 3.9
Commission regulation (EC) No 641/2009
Plastic GF 1.4 %
Commission regulation (EU) No 622/2012
Standards used: EN 16297-1:2012, EN 16297-2:2012. Copper 6.6 %
Ceramic 0.9 %
Iron 41.6 %
RoHS Directives (2011/65/EU) and (2015/863/EU)
Magnet Nd 0.3 %
Standard used: EN IEC 63000:2018.
Electronics 6.0 %
Aluminium 7.3 %
The CE-marking takes into account the proof of conformity with Plastic film 0.2 %
the respective harmonized standards based on the legal Plastic film packaging 0.2
provisions above.
Paper 6.5 %
Cardboard 5.8 %
For the application and use the respective national provisions Rubber 0.2 %
apply. REACH
The product does not contain substances listed in the
Application
Candidate List of Substances of Very High Concern for
Grundfos ALPHA high-efficiency circulator pumps with cast-iron
Authorisation (15.01.2018) exceeding 0.1 percentage by mass.
pump housing are designed for circulating liquids in all kinds of
HVAC systems.
ISO 14001
The Bjerringbro production has been assessed and certified as
Technical Data
meeting the requirements of ISO 14001:2015 (Certificate
The performance data of the product according to the
DE11/81829052.00).
harmonised norms, based on the harmonisation provisions
above apply. The relevant technical specifications according to Reference service life
the PCR Part B are given in the table below. Characteristics
No use stage scenario which refers to the lifetime of the product
that are the same for all three product groups are only given
is declared. However, to facilitate building calculations, an
once. Others are given individually for all three groups.
estimated RSL of 10 years can be used. This is an EU
Constructional data consensus-based estimation, referenced on page 37 in
Appendix 7: Lot 11 – Circulators in Buildings, prepared by AEA
Energy & Environment for the European Commission in the
context of the Eco Design Directive:
2 Environmental Product Declaration - Grundfos Holding A/S - ALPHA2, ALPHA1, ALPHA2 L, ALPHA1.1, ALPHA2.1, ALPHA2.2 (Cast Iron)
There is no definitive information on average circulator life
available, there is consensus within the industry that it is at The RSL of the declared product is not directly influencing the
least 12 years. However, this is complicated by many factors, results in this study, as no declared use stage scenario is
including many being scrapped prematurely when e.g. the dependent on the RSL. The use stage sub-module B6 is
boiler they are connected to is replaced. declared per year as required by the PCR Part B.
LCA: Calculation rules
considered during the application process.
Declared Unit
The declared unit is 1 piece of product, including packaging. Modules B1-B7 refer to the use stage. In this study, all use
Declared unit stage modules are assessed, though B1, B2 and B7 are
assessed to be zero. By decision no. 20170712-n of the SVR,
Name Value Unit
the modules B3, B4 and B5 are by default declared as
Declared unit 1 pce.
"MNR" (module not relevant). The modules include the
Mass reference * 2.21 kg/pce provision and transport of all materials, products and related
conversion factor [Mass/Declared Unit] 2.21 - energy and water use, as well as waste processing up to the
end-of-waste state or disposal of final residues during the use
The weighted average product has been calculated based on
stage. They also include all impacts and aspects related to the
the mass of the inputs of all individual pump modules and their
losses during the use stage (i.e. production, transport, and
production volumes.
waste processing and disposal of the lost products and
materials).
The LCA study to support these results is robust, based on the
inclusion of different production locations, high geographical
Module B6 contributions to operational energy use during the
representativeness and careful selection of background
use stage comes from the electricity consumption of the
datasets, thereby matching modeled production process and
product. The annual electricity consumption is calculated by
the actual production process.
multiplying the average power input, which is based on a
System boundary defined load profile, with the annual running hours.
This LCA is a Cradle-to-Grave study. All major steps from the
Modules C1-C4 refers to the End-of-life stage. A product
extraction of natural resources to the final disposal of the
reaches the end-of-life of its service life when it no longer
product are included in the scope of the analysis, following the
provides any functionality. This life cycle stage includes all
modular approach of EN15804+A2:2019.
activities from the end-of-life of the pump, until all materials and
By decision no. 20170712-n of the SVR, the modules B3, B4
components are processed, reused, recycled or disposed of. In
and B5 are by default declared as "MNR" (module not relevant).
accordance with EN15804+A2 and the PCR Part A C1-C4 are
included.
Modules A1-A3 refer to the product stage and includes raw
materials extraction and processing, transportation and
Module D refers to the burdens and benefits beyond the
distribution, and the manufacturing process. The product stage
system boundaries. According to EN15804:A2+2019 module D
is included in this study, and according to EN 15804:2019 + A2
includes the reuse, recovery and/or recycling potentials,
the system boundary with nature is set to include those
expressed in net impacts and benefits.
processes that provide the material and energy inputs into the
Contributions to module D comes from waste incineration
system and the following manufacturing, transport up to the
processes in A5 and C4 as well as
factory gate as well as the processing of any waste arising from
material recycling in C3. The specific fractions and net flows are
those processes.
shown in the scenarios section.
Wastes and losses are included in the modules where they
occur according to the polluter pays principle and the modular
Geographic Representativeness
approach of EN 15804:2019+A2.
Land or region, in which the declared product system is
manufactured, used or handled at the end of the product´s
Module A4 regards the transportation to the construction place
lifespan: Europe
as well as the transport from the production site to the regional
distribution centre, and finally to the point of sale.
Comparability
Module A5 refers to the construction and installation process of
Basically, a comparison or an evaluation of EPD data is only
the pumps, including the transportation of packaging waste to
possible if all the data sets to be compared were created
the treatment site and the waste treatment of packaging.
according to EN 15804 and the building context, respectively
The use of energy during application (i.e. an electric hand drill)
the product-specific characteristics of performance, are taken
is negligible for the selected functional unit and is therefore not
into account. Software and database used Gabi TS / Ecoinvent
included in the scope of this study. The auxiliary materials are
3.8
considered capital goods. There are no direct emission
LCA: Scenarios and additional technical information
There is biogenic carbon in the cardboard packaging.
Characteristic product properties of biogenic carbon
Information on describing the biogenic carbon content at
The biogenic carbon content quantifies the amount of biogenic
factory gate
carbon in a construction product leaving the factory gate, and it
shall be separately declared for the product and for any
accompanying packaging. In the product there is no biogenic
carbon that exceeds the minimal reporting requirement of 5%.
3 Environmental Product Declaration - Grundfos Holding A/S - ALPHA2, ALPHA1, ALPHA2 L, ALPHA1.1, ALPHA2.1, ALPHA2.2 (Cast Iron)
Name ValueUnit An estimated RSL of 10 years can be used to facilitate building
calculations. This is an EU
kg
Biogenic carbon content in product - consensus-based estimation, referenced in Appendix 7: Lot 11
C
– Circulators in Buildings, prepared by AEA Energy &
Biogenic carbon content in accompanying kg
0.12 Environment for the European Commission in the context of the
packaging C
Eco Design Directive.
Operational energy use (B6)
Note: 1 kg of biogenic carbon is equivalent to 44/12 kg of CO2.
Name Value Unit
The following technical information forms the basis for the
declared gate-to-grave modules and can be used for Electricity consumption Gr 1 46.88 kWh/year
developing specific scenarios in the context of a building Electricity consumption Gr 2 78.85 kWh/year
assessment. Electricity consumption Gr 2 112.63 kWh/year
Transport from the gate to the site (A4)
End of life (C1-C4)
Name Value Unit
Name ValueUnit
Litres of fuel 0.0322 l/100km
Disassembly of the pump 1.85 Kg
Transport distance 500 km
Transport (C2) 500 Km
Capacity utilisation (including empty runs) 85 %
Recycling (cast iron, steel and stainless steel) 1.62 Kg
Gross density of products transported 450 kg/m3
Plastic waste for incineration with energy recovery 0.28 Kg
Assembly (A5) Landfilling 0.15 Kg
Name ValueUnit
Reuse, recovery and/or recycling potentials (D), relevant
Packaging waste for incineration with energy
0.36 Kg scenario information
recovery (plastic, paper and cardboard)
Net scenarios have been used to calculate module D.
As the B6 indicator results for this product only come from the Name Value Unit
electricity consumption dataset, there is a linear correlation
Energy recovery from incineration (A5+C4) -6.67 MJ/Kg
between the product groups based on the electricity
Cast iron, steel and stainless steel recycling -1.62 Kg
consumption. By multiplying the reported impacts of B6 with the
factors in the table below the impacts can be calculated for the
other lifting weigths.
Name Value Unit
Lifting weight 4m factor 1
Lifting weight 6m factor 1.65
Lifting weight 8m factor 2.53
4 Environmental Product Declaration - Grundfos Holding A/S - ALPHA2, ALPHA1, ALPHA2 L, ALPHA1.1, ALPHA2.1, ALPHA2.2 (Cast Iron)
LCA: Results
The LCA results in module B6 are given over a period of one year, according to PCR Part B. To obtain the results from module B6 over
the entire life cycle, the LCA results of module B6 mustbe multiplied by the estimated RSL of 10 years.
DESCRIPTION OF THE SYSTEM BOUNDARY (X = INCLUDED IN LCA; MND = MODULE OR INDICATOR NOT DECLARED; MNR
= MODULE NOT RELEVANT)
Benefits and
Construction loads beyond
Product stage Use stage End of life stage
process stage the system
boundaries
la ire ta m w a Ry lp p u s tro p s n a rT g n iru tc a fu n a M e h t m o rf tro p s n a rTe tis e h t o t e ta g y lb m e s s A e s U e c n a n e tn ia M ria p e R tn e m e c a lp e R tn e m h s ib ru fe R y g re n e la n o ita re p Oe s u re ta w la n o ita re p Oe s u n o itc u rts n o c -e Dn o itilo m e d tro p s n a rT g n is s e c o rp e ts a W la s o p s iD -e s u e R-y re v o c e R-g n ilc y c e Rla itn e to p
A1 A2 A3 A4 A5 B1 B2 B3 B4 B5 B6 B7 C1 C2 C3 C4 D
X X X X X X X X X X X X X X X X X
RESULTS OF THE LCA - ENVIRONMENTAL IMPACT according to EN 15804+A2: 1 Piece Alpha 1/2 pump - Cast Iron
Parameter Unit A1-A3 A4 A5 B1 B2 B3 B4 B5 B6 B7 C1 C2 C3 C4 D
1.45E -1.33E
GWP-total kg CO 2 eq 1.25E+01 2.87E-01 3.95E-01 0 0 MNR MNR MNR +01 0 0 8.19E-02 6.49E-01 5.06E-01 +00
1.43E -1.33E
GWP-fossil kg CO 2 eq 1.34E+01 2.88E-01 1.69E-01 0 0 MNR MNR MNR +01 0 0 8.23E-02 6.5E-01 5.06E-01 +00
GWP-
biogenic kg CO 2 eq-9.36E-01-4.02E-03 2.25E-01 0 0 MNR MNR MNR 1.55E-01 0 0 -1.15E-03-1.07E-03 9.36E-01 -7.65E-04
GWP-luluc kg CO 2 eq 1.47E-02 2.65E-03 1.25E-04 0 0 MNR MNR MNR 1.54E-03 0 0 7.56E-04 3.14E-04 4.7E-06 -2.47E-04
kg CFC11
ODP 2.02E-07 3.72E-14 1.05E-09 0 0 MNR MNR MNR 2.61E-10 0 0 1.06E-14 1.1E-08 1.18E-09 -3.04E-08
eq
AP mol H+ eq 1.88E-01 1.84E-03 1.77E-04 0 0 MNR MNR MNR 3.01E-02 0 0 5.25E-04 1.2E-03 1.18E-04 -3.51E-03
EP-
kg P eq 2.14E-03 1.04E-06 1.17E-05 0 0 MNR MNR MNR 5.3E-05 0 0 2.99E-07 7.6E-05 1.52E-06 -2.79E-04
freshwater
EP-marine kg N eq 5.04E-02 9E-04 8.95E-05 0 0 MNR MNR MNR 7.22E-03 0 0 2.57E-04 3.08E-04 6.63E-05 -9.37E-04
EP-terrestrial mol N eq 1.59E-01 9.96E-03 8.68E-04 0 0 MNR MNR MNR 7.55E-02 0 0 2.85E-03 3.12E-03 5.67E-04 -1E-02
kg
POCP NMVOC 4.93E-02 1.74E-03 1.83E-04 0 0 MNR MNR MNR 1.93E-02 0 0 4.97E-04 8.2E-04 1.38E-04 -4.46E-03
eq
ADPE kg Sb eq 1.76E-03 1.88E-08 3.23E-08 0 0 MNR MNR MNR 2.19E-06 0 0 5.38E-09 6.36E-06 3.63E-08 -6.14E-07
2.97E -2.07E
ADPF MJ 1.81E+02 3.89E+00 2.77E-01 0 0 MNR MNR MNR 0 0 1.11E+00 2.29E+00 1.08E-01
+02 +01
m3 world
-3.13E
WDP eq 3.45E-03 1.51E-02 0 0 MNR MNR MNR 3.11E+00 0 0 9.87E-04 5.33E-02 3.24E-02 -1.06E-01
+01
deprived
GWP = Global warming potential; ODP = Depletion potential of the stratospheric ozone layer; AP = Acidification potential of land and water; EP =
Eutrophication potential; POCP = Formation potential of tropospheric ozone photochemical oxidants; ADPE = Abiotic depletion potential for non-fossil
resources; ADPF = Abiotic depletion potential for fossil resources; WDP = Water (user) deprivation potential)
RESULTS OF THE LCA - INDICATORS TO DESCRIBE RESOURCE USE according to EN 15804+A2: 1 Piece Alpha 1/2 pump -
Cast Iron
Parameter Unit A1-A3 A4 A5 B1 B2 B3 B4 B5 B6 B7 C1 C2 C3 C4 D
PERE MJ 4.95E+01 2.83E-01 1.58E-02 0 0 MNR MNR MNR 1.78E+02 0 0 8.1E-02 2.34E-01 3.74E-03 -3.1E+00
PERM MJ 2.88E-06 3.73E-12 1.89E-09 0 0 MNR MNR MNR 4.86E-08 0 0 1.06E-12 3.79E-08 1.6E-09 -1.1E-07
PERT MJ 4.95E+01 2.83E-01 1.58E-02 0 0 MNR MNR MNR 1.78E+02 0 0 8.1E-02 2.34E-01 3.74E-03 -3.1E+00
-2.07E
PENRE MJ 1.81E+02 3.91E+00 2.77E-01 0 0 MNR MNR MNR 2.97E+02 0 0 1.12E+002.29E+00 1.08E-01
+01
PENRM MJ 1.75E-03 4.64E-08 2.08E-09 0 0 MNR MNR MNR 7.17E-07 0 0 1.33E-08 0 0 -2.14E-08
-2.07E
PENRT MJ 1.81E+02 3.91E+00 2.77E-01 0 0 MNR MNR MNR 2.97E+02 0 0 1.12E+002.29E+00 1.08E-01
+01
SM kg 1.19E+00 0 0 0 0 MNR MNR MNR 0 0 0 0 0 0 0
RSF MJ 0 0 0 0 0 MNR MNR MNR 0 0 0 0 0 0 0
NRSF MJ 0 0 0 0 0 MNR MNR MNR 0 0 0 0 0 0 0
FW m3 -7.07E-01 3.1E-04 3.61E-04 0 0 MNR MNR MNR 1.43E-01 0 0 8.87E-05 1.24E-03 7.54E-04 -3.64E-03
PERE = Use of renewable primary energy excluding renewable primary energy resources used as raw materials; PERM = Use of renewable primary
energy resources used as raw materials; PERT = Total use of renewable primary energy resources; PENRE = Use of non-renewable primary energy
excluding non-renewable primary energy resources used as raw materials; PENRM = Use of non-renewable primary energy resources used as raw
materials; PENRT = Total use of non-renewable primary energy resources; SM = Use of secondary material; RSF = Use of renewable secondary fuels;
NRSF = Use of non-renewable secondary fuels; FW = Use of net fresh water
RESULTS OF THE LCA – WASTE CATEGORIES AND OUTPUT FLOWS according to EN 15804+A2:
1 Piece Alpha 1/2 pump - Cast Iron
5 Environmental Product Declaration - Grundfos Holding A/S - ALPHA2, ALPHA1, ALPHA2 L, ALPHA1.1, ALPHA2.1, ALPHA2.2 (Cast Iron)
Parameter Unit A1-A3 A4 A5 B1 B2 B3 B4 B5 B6 B7 C1 C2 C3 C4 D
HWD kg 8.57E-07 1.21E-11 5.44E-13 0 0 MNR MNR MNR -2.32E-08 0 0 3.46E-12 0 0 -5.03E-11
NHWD kg 3.59E-01 0 3.62E-01 0 0 MNR MNR MNR 0 0 0 0 0 2.4E-01 0
RWD kg 5.43E-03 7.31E-06 3.29E-07 0 0 MNR MNR MNR 4.71E-02 0 0 2.09E-06 0 0 -7.81E-04
CRU kg ND ND ND ND ND ND ND ND ND ND ND ND ND ND ND
1.62E
MFR kg 0 0 0 0 0 MNR MNR MNR 0 0 0 0 0 0
+00
MER kg 0 0 3.13E-01 0 0 MNR MNR MNR 0 0 0 0 0 6.79E-02 0
EEE MJ 0 0 4.35E-01 0 0 MNR MNR MNR 0 0 0 0 0 2.66E-01 0
EET MJ 0 0 8.92E-01 0 0 MNR MNR MNR 0 0 0 0 0 5.2E-01 0
HWD = Hazardous waste disposed; NHWD = Non-hazardous waste disposed; RWD = Radioactive waste disposed; CRU = Components for re-use;
MFR = Materials for recycling; MER = Materials for energy recovery; EEE = Exported electrical energy; EET = Exported thermal energy
RESULTS OF THE LCA – additional impact categories according to EN 15804+A2-optional:
1 Piece Alpha 1/2 pump - Cast Iron
Parameter Unit A1-A3 A4 A5 B1 B2 B3 B4 B5 B6 B7 C1 C2 C3 C4 D
Disease
PM 1.7E-06 6.82E-09 1.11E-09 0 0 MNR MNR MNR 2.54E-07 0 0 1.95E-09 1.19E-08 5.74E-10 -5.28E-08
incidence
kBq U235
IR 1.21E+001.09E-03 3.56E-04 0 0 MNR MNR MNR 7.83E+00 0 0 3.12E-04 1.68E-02 3.11E-04 -1.43E-01
eq
-2.44E
ETP-fw CTUe 6E+02 2.77E+00 9.6E-01 0 0 MNR MNR MNR 1.31E+02 0 0 7.9E-01 7.85E+001.07E+00
+01
HTP-c CTUh 1.4E-08 5.66E-11 4.83E-11 0 0 MNR MNR MNR 4.37E-09 0 0 1.62E-11 2.08E-10 4.58E-11 -3.9E-09
HTP-nc CTUh 3.76E-07 3.22E-09 1.78E-09 0 0 MNR MNR MNR 1.07E-07 0 0 9.2E-10 1.88E-08 1.73E-09 -1.83E-08
-3.48E
SQP SQP 9.04E+011.63E+00 1.4E-01 0 0 MNR MNR MNR 1.17E+02 0 0 4.65E-01 1.6E+00 4.2E-02
+00
PM = Potential incidence of disease due to PM emissions; IR = Potential Human exposure efficiency relative to U235; ETP-fw = Potential comparative
Toxic Unit for ecosystems; HTP-c = Potential comparative Toxic Unit for humans (cancerogenic); HTP-nc = Potential comparative Toxic Unit for humans
(not cancerogenic); SQP = Potential soil quality index
Disclaimer 1 – for the indicator “Potential Human exposure efficiency relative to U235”. This impact category deals mainly with the
eventual impact of low-dose ionizing radiation on human health of the nuclear fuel cycle. It does not consider effects due to possible
nuclear accidents, occupational exposure or radioactive waste disposal in underground facilities. Potential ionizing radiation from the
soil, radon and from some construction materials is also not measured by this indicator.
Disclaimer 2 – for the indicators “abiotic depletion potential for non-fossil resources”, “abiotic depletion potential for fossil resources”,
“water (user) deprivation potential, deprivation-weighted water consumption”, “potential comparative toxic unit for ecosystems”,
“potential comparative toxic unit for humans – cancerogenic”, “Potential comparative toxic unit for humans - not cancerogenic”,
“potential soil quality index”. The results of this environmental impact indicator shall be used with care as the uncertainties on these
results are high as there is limited experience with the indicator.
This EPD was created using a software tool.
References
Standards
Sphera LCA for Experts
Sphera LCA for Experts Software-System and Database for Life
EN 15804 Cycle Engineering. Copyright 1992-2023 Sphera (version
EN 15804:2012+A1 2013, Sustainability of construction works 10.7.0.183)
— Environmental Product Declarations — Core rules for the
product category of construction products.
IBU 2021
EN 15804 Institut Bauen und Umwelt e.V.: General Instructions for the
EN 15804:2012+A2:2019+AC:2021, Sustainability of EPD programme of Institut Bauen und Umwelt e.V., Version
construction works — Environmental Product Declarations — 2.0, Berlin: Institut Bauen und Umwelt e.V., 2021
Core rules for the product category of construction products. www.ibu-epd.com
Low Voltage Directive (2014/35/EU)
ISO 14001 EN 60335-1:2012/A15:2021 Household and similar electrical
EN ISO 14001:2015-09 Environmental management systems - appliances – Safety – Part I: General requirements; EN 60335-
Requirements with guidance for use 2-51:2003/A2:2012 Household and similar electrical appliances
– Safety – Part 2-51: Particular requirements for stationary
circulation pumps for heating and service water installations.
ISO 14025
EN ISO 14025:2011, Environmental labels and declarations —
Type III environmental declarations — Principles and EMC Directive (2014/30/EU)
procedures. EN 55014-1:2017 Electromagnetic compatibility –
Requirements for household appliances, electric tools and
similar apparatus – Part 1: Emission; EN 55014-2:2015
Further References Electromagnetic compatibility – Requirements for household
appliances, electric tools and similar apparatus – Part 2:
6 Environmental Product Declaration - Grundfos Holding A/S - ALPHA2, ALPHA1, ALPHA2 L, ALPHA1.1, ALPHA2.1, ALPHA2.2 (Cast Iron)
Immunity – Product family standards; EN IEC 61000-3-2:2019 assessment of electrical and electronic products with respect to
Electromagnetic compatibility (EMC) – Part 3-2: Limits – Limits the restriction of hazardous substances.
for harmonic current emissions (equipment input current ≤16 A
per phase); EN 61000-3-3:2013 Electromagnetic compatibility
(EMC) – Part 3-3: Limits – Limitation of voltage changes,
voltage fluctuations and flicker in public low voltage supply
systems, for equipment with rated current ≤16 A per phase and IBU 2022
not subject to conditional connection. Product Category Rules for Building-Related Products and
Services, Part A: Calculation Rules for the Life Cycle
Assessment and Requirements on the Project Report according
Ecodesign Directive (2009/125/EC) to EN15804+A2:2019, Version 1.3.
Commission regulation (EC) No 641/2009
Commission regulation (EU) No 622/2012 IBU 2022
EN 16297-1:2012 Pumps – Rotodynamic pumps – Glandless
circulators – Part I: General requirements and procedures for PCR Guidance-Text for Building-Related Products and
testing and calculation of energy efficiency index (EEI); EN Services, Part B: Requirements on the EPD for Pumps for
16297-2:2012 Pumps – Rotodynamic pumps – Glandless liquids and with solids, Version 1.0.
circulators – Part 2: Calculation of energy efficiency index (EEI) Circulators in Buildings, prepared by AEA Energy &
for standalone circulators. Environment [BSJ1] for the European Commission in the
context of the Eco Design Directive.
RoHS Directives (2011/65/EU) and (2015/863/EU)
EN IEC 63000:2018 Technical documentation for the
7 Environmental Product Declaration - Grundfos Holding A/S - ALPHA2, ALPHA1, ALPHA2 L, ALPHA1.1, ALPHA2.1, ALPHA2.2 (Cast Iron)
Publisher
Institut Bauen und Umwelt e.V. +49 (0)30 3087748- 0
Hegelplatz 1 info@ibu-epd.com
10117 Berlin www.ibu-epd.com
Germany
Programme holder
Institut Bauen und Umwelt e.V. +49 (0)30 3087748- 0
Hegelplatz 1 info@ibu-epd.com
10117 Berlin www.ibu-epd.com
Germany
Author of the Life Cycle Assessment
Ecomatters BV +31 6 44836384
Weg der Verenigde Naties 1 info@ecomatters.nl
3527TK Utrecht https://www.ecomatters.nl/
Netherlands
Owner of the Declaration
Grundfos Holding A/S +45 87501400
Poul Due Jensens Vej 7 LCA_EPD@grundfos.com
8850 Bjerringbro www.grundfos.com
Denmark
8 Environmental Product Declaration - Grundfos Holding A/S - ALPHA2, ALPHA1, ALPHA2 L, ALPHA1.1, ALPHA2.1, ALPHA2.2 (Cast Iron)
