ENVIRONMENTAL PRODUCT DECLARATION
as per ISO 14025 and EN 15804+A1
Owner of the Declaration Isolparma
Programme holder Institut Bauen und Umwelt e.V. (IBU)
Publisher Institut Bauen und Umwelt e.V. (IBU)
Declaration number EPD-ISL-20200306-CBA2-EN
Issue date 18.12.2020
Valid to 17.12.2025
ISOLPARMA Pendenzato RF8 average thick panel
Isolparma
www.ibu-epd.com | https://epd-online.com
Umwelt Produktdeklaration Name des Herstellers – Name des Produkts
General Information
Isolparma ISOLPARMA Pendenzato RF8
insulation panel
Programme holder Owner of the declaration
IBU – Institut Bauen und Umwelt e.V. Isolparma
Panoramastr. 1 Piazza L. Da Porto, n. 14
10178 Berlin
Germany 35131 | Padova | PD | Italy
Declaration number Declared product / declared unit
EPD-ISL-20200306-CBA2-EN ISOLPARMA Pendenzato RF8 is a composite panel
made by a base side by EPS and a top side based on
ISOLPARMA RF8, expanded rigid polyurethane foam,
covered on top side by bituminous glass fibres, and
produced by Isolparma. The EPD applies to 1 m2 of a
average 122 mm thick PUR sandwich board, i.e. 0.122
m3, with an average density between foam and facing
of 32.1 kg/m3.
This declaration is based on the product Scope:
category rules: Isolparma produces ISOLPARMA Pendenzato RF8 is
Insulating materials made of foam plastics, 06.2017 a composite panel made by a base side by EPS and a
(PCR checked and approved by the SVR) top side based on Isolparma RF8, expanded rigid
polyurethane foam, covered on top side by bituminous
glass fibres.The data have been provided by the only
Issue date
Isolparma factory that was located in Padova (Italy) for
18.12.2020
the year 2019.The owner of the declaration shall be
liable for the underlying information and evidence; the
Valid to IBU shall not be liable with respect to manufacturer
17.12.2025 information, life cycle assessment data and evidences.
The owner of the declaration shall be liable for the
underlying information and evidence; the IBU shall not
be liable with respect to manufacturer information, life
cycle assessment data and evidences.
The EPD was created according to the specifications
of EN 15804+A1. In the following, the standard will be
simplified as EN 15804.
Verification
The standard EN 15804 serves as the core PCR
Independent verification of the declaration and data
according to ISO 14025:2010
Dipl. Ing. Hans Peters internally x externally
(chairman of Institut Bauen und Umwelt e.V.)
Dr. Alexander Röder Prof. Dr. Birgit Grahl
(Managing Director Institut Bauen und Umwelt e.V.)) (Independent verifier)
Product
Product description/Product definition The performance of Isolparma’s panels is determined
Isolparma's thermo insulation panels are mainly used based on the European norm EN
in the building/construction sector or industrial 13165:2012+A2:2016 Thermal insulation products for
insulation. buildings - Factory made rigid polyurethane foam (PU)
The panels are made of thermo-setting closed cells products - Specification/ for polyurethane insulation
polyurethane foam (PU) supplied with various types of board and on the European norm EN
flexible facers on both sides of the panel. The 13163:2012+A2:2016 Thermal insultaion for building-
nature/type of facer contributes to the performance factory made expanded polystyrene (EPS) products -
characteristics of the product and its application. Specification for polystyrene insulation board.
Expanded rigid polyurethane foam is distinguished by This EPD refers to Isolparma PENDENZATO RF8
its good thermo insulation performance, mechanical Average thick panel, made of an insulation component
resistance, workability, lightness, and durability. in polyurethane foam using blowing agent Pentane-
2 Environmental Product Declaration Isolparma srl – Isolparma Pendenzato RF8
based, covered on top side by bituminous glass fibers,
and on the bottom side of an insulation component in Base materials/Ancillary materials
EPS with a slope shape. PU insulation panel (about 53,1 % of the weight of
the declared unit):
Closed-cell Polyiso (PIR) rigid foam made from MDI
The panel is produced in standard dimensions of as (50-65%), polyols (20-30 %), pentane (4-5%) and
request by the customers and straight finish borders. additives (4-7%).
The surface of the panel may be evened off by PU Facing (about 14,6 % of the weight of the
sandpaper in order to allow installation to uneven declared unit): upper and lower facing consisting of
surfaces. Isolparma PENDENZATO RF8 Average bitumen (40-60 %), PP (4-10 %), urea-formaldehyde
thick panel is produced by a certified company with (1-5 %), calcium carbonate (1-5%) and glass fibre (30-
systems: ISO 9001, ISO 45001, ISO 14001 in its entire 40 %).
line of products. EPS insulation panels: about 32,3 %
For the placing on the market of the product in the The PU board for insulation:
EuropeanUnion/European Free Trade Association o This product/article/at least one
(EU/EFTA) (with the exception of Switzerland) partial article contains substances
Regulation (EU) No. 305/2011 (CPR) applies. The
listed in the candidate list (date:
product needs a declaration of perfomance taking into
17.11.2020) exceeding 0.1
consideration for polyurethane side EU
percentage by mass: no
13165:2012+A2:2016 Thermal insultaion for building-
factory made rigid polyurethane foam (PU) products – o This product/article/at least one
Specification and the CE marking, and for EPS side partial article doesn’t contain other
EN 13163:2012+A2:2016 Thermal insultaion for CMR substances in categories 1A or
building-factory made expanded polystyrene (EPS) 1B which are not on the candidate
products– Specification and the CE marking. For the
list, exceeding 0.1 percentage by
application and use the respective national provisions
mass: no
apply.
Application o Biocide products were added to this
The Isolparma Pendenzato RF8 panel is suited for construction product or it has been
roofs under bituminous waterproofing mantles and treated with biocide products (this
where high resistance to a flame torch is required. then concerns a treated product as
defined by the (EU) Ordinance on
Technical Data
Biocide Products No. 528/2012): no
The data provided by the Declaration of Performance
apply. In this Life Cycle Assessment, a PU insulation
board with the following properties has been regarded: Additional declaration according to quoted law: The
product is compliant with all requirements indicated at
Constructional data chapter 2.4.2.9 of the PANGPP 2017:
Name Value Unit  Any blowing agent with Ozone depletion
Gross density 32.1 kg/m3 potential >0 is not used in production
PU:0.02  Catalysts lead-based are not used in
Declared Average Thermal 7,
W/mK production
conductivity λD acc. to /EN 13165/ EPS:0.0
 Flame retardants used in production
33
Compressive strength at 10% (belonging to the Organophosphorus class)
> 150 kPa
deformation acc. to /EN 826/ are not banned by any national or European
Tensile strength perpendicular to the regulation
> 40 kPa
face acc. to /EN 1607/  According to the raw materials declarations of
Water absorption by total immersion
< 2 Vol.-% suppliers the minimum amount of recycled
acc. to /EN 12087/
raw materials based on the insulation board
Water absorption by partial immersion
< 0.1 kg/m² (PU foam and facers) weight is 3 %w and the
acc. to /EN 1609/
minimum amount of recycled raw materials
PU:33,
Water vapour diffusion resistance
EPS:30- based on the PU insulation foam weight is 4
factor μ acc. to /EN 12086/
70 %w (note: this information is not explicitly
Euroclass reaction to fire acc. to /EN considered in the LCA and not included in the
F
11925/ EPD tables that only refer to recycling content
in the foreground system).
This provides a thermal resistance R = 4.14 m² k/W.
The LCI data used in this report refer to an average
product having an average thickness (materials in the Reference service life
recipes of different thicknesses are weighted according The durability of insulation panels is normally at least
to the relative production in square meters). The type as long as the lifetime of the building in which it is
of declaration is 1 c - declaration of an average product used. The experimental data show that the reference
from a manufacturer's plant. life is longer than 50 years, Clima 2019.
3 Environmental Product Declaration Isolparma srl – Isolparma Pendenzato RF8
LCA: Calculation rules
Declared Unit the end-of-life stage of the used PU thermal insulation
The declared unit is 1 m² with an average thickness of board. The life cycle is split into the following individual
122 mm, e. g. 0.122 m³. Corresponding conversion phases:
factors are listed in the table below. A1 - Raw material formulation
A2 - Raw material transport
Declared unit A3 - Production of the insulation board and packaging
Name Value Unit material
Declared unit 1 m2 A4 - Transport to the construction site
Gross density 32.1 kg/m3 A5 - Emissions and cutting losses during installation
Volume 0.122 m³ and packaging disposal
Grammage 3.92 kg/m2 C2 - Transport to end-of-life
Declared average thermal PU:0.027, C3/C4 - End-of-Life: waste management (thermal
W/mK
conductivity λD EPS:0.033 recovery, landfill)
Layer thickness 0.112 m D - Benefits and loads beyond system boundary
Conversion factor to 1 kg 3.92 kg/m²
Comparability
Weight of declared unit 3.92 kg/m²
Basically, a comparison or an evaluation of EPD data
is only possible if all the data sets to be compared
This provides a thermal resistance R = 4.14 m² /W.
were created according to EN 15804 and the building
context, respectively the product-specific
The LCI data used in this report refer to an average
characteristics of performance, are taken into account.
product having an average thickness (materials in the
recipes of different thicknesses are weighted according
For life cycle modelling of the considered products,
to the relative production in square meters). The type
the GaBi 9 2020 has been used.
of declaration is 1 c - declaration of an average product
from a manufacturer's plant.
System boundary
This life cycle assessment for the production of the
polyurethane insulation board considers the life cycle
from the supply of raw materials to the manufacturer´s
gate (cradle-to-gate with options). It also includes the
transport to the construction site, the installation and
LCA: Scenarios and additional technical information
RSL
Water consumption - m3
Transport to the building site (A4) Auxiliary - kg
The distances calculated are weighted average Other resources - kg
distances according to the overall sales distribution; Electricity consumption - kWh
such distribution is considered similar for all Isolparma Other energy carriers - MJ
products.
Material loss - kg
Name Value Unit
Truck with a capacity of 17.3 tons 270 km
Repair (B3)
Ferry with a capacity of 1200-10000
124 km Name Value Unit
dwt payload capacity
Information on the repair process - -
Ship with a capacity of 27500 dwt
11000 km Information on the inspection process - -
payload capacity tons
Number/
Plane with a capacity of 22 ton 0 km Repair cycle -
RSL
Water consumption - m3
Installation into the building (A5)
Auxiliary - kg
Name Value Unit
Other resources - kg
Material loss 0.0784 kg
Electricity consumption - kWh
VOC in the air Pentane 1.27E-06 kg
Other energy carriers - MJ
Material loss - kg
Use or application of the installed product (B1) see
Replacement (B4) / Refurbishment (B5)
section 2.12 "Use"
Name Value Unit
Name Value Unit
Number/
Replacement cycle -
RSL
Maintenance (B2)
Electricity consumption - kWh
Name Value Unit
Litres of fuel - l/100km
Information on maintenance - -
Replacement of worn parts - kg
Maintenance cycle - Number/
4 Environmental Product Declaration Isolparma srl – Isolparma Pendenzato RF8
Reference service life
Name Value Unit
Reference service life - a
Life Span (according to BBSR) - a
Life Span according to the
- a
manufacturer
Declared product properties (at the
- -
gate) and finishes
Design application parameters (if
instructed by the manufacturer),
including the references to the - -
appropriate practices and application
codes
An assumed quality of work, when
installed in accordance with the - -
manufacturer’s instructions
Outdoor environment, (for outdoor
applications), e.g. weathering,
pollutants, UV and wind exposure, - -
building orientation, shading,
temperature
Indoor environment (for indoor
applications), e.g. temperature, - -
moisture, chemical exposure
Usage conditions, e.g. frequency of
- -
use, mechanical exposure
Maintenance e.g. required frequency,
type and quality and replacement of - -
components
Operational energy use (B6) and Operational water
use (B7)
Name Value Unit
Water consumption - m3
Electricity consumption - kWh
Other energy carriers - MJ
Equipment output - kW
End of life (C1-C4)
The results for the end-of-life are declared for the 2
different scenarios:
Name Value Unit
Scenario No 1: Material Incineration 100 %
Scenario No 2: Landfill 100 %
C4: Disposal scenarios used is divided into the 2
sub-scenarios:
1) Incineration 100% (C4/1)
2) Landfilling 100% (C4/2)
D: Benefits and loads beyond system boundary are
divided into the 2 sub-scenarios:
1) Incineration 100% (D1)
2) Landfilling 100% (D2)
Reuse, recovery and/or recycling potentials (D),
relevant scenario information
Name Value Unit
Module D includes credits from recycling materials of
insulation panels and packaging, energy credits from
thermal recovery of the packaging. The results are
declared for the same 3 different scenarios described
above.
5 Environmental Product Declaration Isolparma srl – Isolparma Pendenzato RF8
LCA: Results
The tables below show the results of the LCA.
There are two scenarios for the end-of-life (C3, C4 and D) analyzed: Scenario 1 considers 100% incineration,
Scenario 2 considers 100% landfill disposal.
For (SM, RSF, NRSF,CRU) indicators only the foreground system is considered.
DESCRIPTION OF THE SYSTEM BOUNDARY (X = INCLUDED IN LCA; MND = MODULE NOT DECLARED;
MNR = MODULE NOT RELEVANT)
BENEFITS AND
CONSTRUCTI LOADS
PRODUCT STAGE ON PROCESS USE STAGE END OF LIFE STAGE BEYOND THE
STAGE SYSTEM
BOUNDARIES
6 Environmental Product Declaration Isolparma srl – Isolparma Pendenzato RF8
lairetam
waR
ylppus tropsnarT
gnirutcafunaM
eht
morf
tropsnarT
etis
eht
ot
etag
ylbmessA esU
ecnanetniaM
riapeR
tnemecalpeR tnemhsibrufeR
ygrene
lanoitarepO esu
retaw
lanoitarepO esu
noitcurtsnoc-eD
noitilomed tropsnarT
gnissecorp
etsaW
lasopsiD -esueR -yrevoceR -gnilcyceR laitnetop
A1 A2 A3 A4 A5 B1 B2 B3 B4 B5 B6 B7 C1 C2 C3 C4 D
X X X X X MND MND MNR MNR MNR MND MND MND X X X X
RESULTS OF THE LCA - ENVIRONMENTAL IMPACT according to EN 15804+A1: 1 m² PENDENZATO RF8
average thickness panel
Parameter Unit A1-A3 A4 A5 C2 C3/1 C3/2 C4/1 C4/2 D/1 D/2
GWP [kg CO2-Eq.] 9.72E+0 7.36E-2 2.51E-1 1.84E-2 0.00E+0 0.00E+0 7.88E+0 4.46E-1 -3.79E+0 -4.42E-2
ODP [kg CFC11-Eq.] 1.00E-5 1.62E-17 2.00E-7 4.57E-18 0.00E+0 0.00E+0 5.53E-15 3.68E-15 -6.84E-14 -6.24E-16
AP [kg SO2-Eq.] 2.22E-2 6.69E-4 4.94E-4 4.04E-5 0.00E+0 0.00E+0 3.02E-3 8.86E-4 -5.61E-3 -5.47E-5
EP [kg (PO4)3--Eq.] 2.86E-3 8.97E-5 6.99E-5 9.81E-6 0.00E+0 0.00E+0 6.14E-4 3.24E-4 -6.74E-4 -7.35E-6
POCP [kg ethene-Eq.] 1.25E-2 -1.27E-5 2.52E-4 -1.30E-5 0.00E+0 0.00E+0 1.77E-4 7.05E-5 -4.73E-4 -6.38E-6
ADPE [kg Sb-Eq.] 3.39E-5 5.64E-9 6.87E-7 1.69E-9 0.00E+0 0.00E+0 3.82E-7 1.58E-7 -8.44E-7 -1.02E-8
ADPF [MJ] 2.52E+2 9.77E-1 5.24E+0 2.49E-1 0.00E+0 0.00E+0 4.24E+0 3.35E+0 -5.14E+1 -1.06E+0
GWP = Global warming potential; ODP = Depletion potential of the stratospheric ozone layer; AP = Acidification potential of land and water; EP =
Caption Eutrophication potential; POCP = Formation potential of tropospheric ozone photochemical oxidants; ADPE = Abiotic depletion potential for non-
fossil resources; ADPF = Abiotic depletion potential for fossil resources
RESULTS OF THE LCA - INDICATORS TO DESCRIBE RESOURCE USE according to EN 15804+A1: 1 m²
PENDENZATO RF8 average thickness panel
Parameter Unit A1-A3 A4 A5 C2 C3/1 C3/2 C4/1 C4/2 D/1 D/2
PERE [MJ] 1.16E+1 IND 2.66E-1 IND IND IND 1.32E+0 IND IND IND
PERM [MJ] 0.00E+0 IND 0.00E+0 IND IND IND 0.00E+0 IND IND IND
PERT [MJ] 1.16E+1 4.46E-2 2.66E-1 1.44E-2 0.00E+0 0.00E+0 1.32E+0 9.56E-1 -1.82E+1 -1.36E-1
PENRE [MJ] 1.19E+2 IND 1.94E+0 IND IND IND 1.48E+2 IND IND IND
PENRM [MJ] 1.44E+2 IND -1.72E+0 IND IND IND -1.43E+2 IND IND IND
PENRT [MJ] 2.63E+2 9.81E-1 2.21E-1 2.50E-1 0.00E+0 0.00E+0 5.21E+0 4.04E+0 -6.70E+1 -1.14E+0
SM [kg] 0.00E+0 0.00E+0 0.00E+0 0.00E+0 0.00E+0 0.00E+0 0.00E+0 0.00E+0 0.00E+0 0.00E+0
RSF [MJ] 0.00E+0 0.00E+0 0.00E+0 0.00E+0 0.00E+0 0.00E+0 0.00E+0 0.00E+0 0.00E+0 0.00E+0
NRSF [MJ] 0.00E+0 0.00E+0 0.00E+0 0.00E+0 0.00E+0 0.00E+0 0.00E+0 0.00E+0 0.00E+0 0.00E+0
FW [m³] 6.09E-2 5.25E-5 1.36E-3 1.68E-5 0.00E+0 0.00E+0 1.97E-2 1.06E-3 -2.10E-2 -1.87E-4
PERE = Use of renewable primary energy excluding renewable primary energy resources used as raw materials; PERM = Use of
renewable primary energy resources used as raw materials; PERT = Total use of renewable primary energy resources; PENRE = Use of
non-renewable primary energy excluding non-renewable primary energy resources used as raw materials; PENRM = Use of non-
Caption
renewable primary energy resources used as raw materials; PENRT = Total use of non-renewable primary energy resources; SM = Use
of secondary material; RSF = Use of renewable secondary fuels; NRSF = Use of non-renewable secondary fuels; FW = Use of net fresh
water
RESULTS OF THE LCA – WASTE CATEGORIES AND OUTPUT FLOWS according to EN 15804+A1:
1 m² PENDENZATO RF8 average thickness panel
Parameter Unit A1-A3 A4 A5 C2 C3/1 C3/2 C4/1 C4/2 D/1 D/2
HWD [kg] 1.06E-3 3.53E-8 2.11E-5 1.16E-8 0.00E+0 0.00E+0 9.71E-9 1.52E-8 -2.65E-8 -3.77E-10
NHWD [kg] 2.01E-1 1.43E-4 9.82E-2 3.97E-5 0.00E+0 0.00E+0 7.72E-1 3.88E+0 -3.36E-2 -3.58E-4
RWD [kg] 4.39E-3 1.65E-6 9.96E-5 4.61E-7 0.00E+0 0.00E+0 3.82E-4 2.72E-4 -6.20E-3 -3.47E-5
CRU [kg] 0.00E+0 0.00E+0 0.00E+0 0.00E+0 0.00E+0 0.00E+0 0.00E+0 0.00E+0 0.00E+0 0.00E+0
MFR [kg] 0.00E+0 0.00E+0 1.37E-2 0.00E+0 0.00E+0 0.00E+0 0.00E+0 0.00E+0 0.00E+0 0.00E+0
MER [kg] 0.00E+0 0.00E+0 1.56E-2 0.00E+0 0.00E+0 0.00E+0 3.92E+0 0.00E+0 0.00E+0 0.00E+0
EEE [MJ] 0.00E+0 0.00E+0 8.65E-2 0.00E+0 0.00E+0 0.00E+0 2.06E+1 0.00E+0 0.00E+0 0.00E+0
EET [MJ] 0.00E+0 0.00E+0 1.56E-1 0.00E+0 0.00E+0 0.00E+0 1.96E+1 0.00E+0 0.00E+0 0.00E+0
HWD = Hazardous waste disposed; NHWD = Non-hazardous waste disposed; RWD = Radioactive waste disposed; CRU = Components
Caption for re-use; MFR = Materials for recycling; MER = Materials for energy recovery; EEE = Exported electrical energy; EET = Exported
thermal energy
References
Standards ISO 9001
ISO 9001:2015 Quality management
EN 15804
EN 15804:2012-04+A1 2013, Sustainability of ISO 14001
construction works — Environmental Product ISO 14001: 2015 Environmental management
Declarations — Core rules for the product category of systems
construction products.
ISO 45001
ISO 14025 ISO 45001: 2018 Occupational health and safety
EN ISO 14025:2011-10, Environmental labels and management systems
declarations — Type III environmental declarations —
Principles and procedures.
Further References
IBU 2016
Institut Bauen und Umwelt e.V.: General Programme BNB
Instructions for the Preparation of EPDs at the Institut Bewertungssystem Nachhaltiges Bauen (en:
Bauen und Umwelt e.V. Version 1., Berlin: Institut assessment system sustainable Building)
Bauen und Umwelt e.V., 2016. https://www.bbsr.bund.de/BBSR/EN/RP/FutureBuilding
www.ibu-epd.com /2SustainableBuildingQuality/2009/ServiceLife/01_Star
t_dossier.html?nn=391866&notFirst=true&docId=3909
EN 13163 00
EN 13163:2012+A2:2016 Thermal insultaion for
building-factory made expanded polystyrene (EPS) Candidate List
products - Specification https://echa.europa.eu/it/candidate-list-table (date
17.11.2020)
EN 13165
EN 13165:2012+A2:2016 Thermal insulation products Clima 2019
for buildings - Clima 2019 PaperPolyurethane
Factory made rigid polyurethane foam (PU) products - “Environmental Impacts for a Polyurethane Panel”
Specification E. Guolo, F. Cappelletti, P. Romagnoni, F. Raggiotto
EN 826 GaBi 9 2020
EN 826:2013 Determination of Compression Behavior GaBi 9: Documentation of GaBi 9: Software-System
of Thermal Insulation Products and Database for Life Cycle Engineering. Copyright,
TM. Stuttgart, Leinfelden-Echterdingen, 1992-2020
EN 1607 http://www.gabi-software.com
EN 1607: 2013 Thermal insulating products for
building applications. Determination of tensile strength PANGPP 2017
perpendicular to faces Piano d’ Azione Nazionale sul Green Public
Procurement (PANGPP) – Gazzetta Ufficiale della
EN 12087 Repubblica Italiana, Serie Generale n.17, 11-10-2017,
EN 12087:2013 http://www.minambiente.it/sites/default/files/archivio/all
Thermal insulating products for building applications. egati/GPP/GPP_CAM_Edilizia.pdf
Determination of long term water absorption by
immersion. PCR Part A
Product Category Rules for Building-Related Products
EN 1609 and Services.
EN 1609: Part A: Calculation Rules for the Life Cycle
Thermal insulating products for building applications. Assessment and Requirements on the Background
Determination of short term water absorption by partial Report. Version 06.2017
immersion.
PCR Part B
EN 12086 PCR Guidance-Texts for Building-Related Products
EN 12086:2013 and Services; Part B: Requirements on the EPD for
Thermal insulating products for building applications. Insulating materials made of foam plastics; Institute
Determination of water vapour transmission properties. Construction and Environment e.V. (IBU). Version
06.2017
EN 11925 https://epd-online.com
EN 11925:2010
Reaction to fire tests. Ignitability of products subjected REACH
to direct impingement of flame. Single-flame source REACH Registration, Evaluation, Authorization and
test. Restriction of Chemical, 2007
7 Environmental Product Declaration Isolparma srl – Isolparma Pendenzato RF8
Publisher
Institut Bauen und Umwelt e.V. Tel +49 (0)30 3087748- 0
Panoramastr. 1 Fax +49 (0)30 3087748- 29
10178 Berlin Mail info@ibu-epd.com
Germany Web www.ibu-epd.com
Programme holder
Institut Bauen und Umwelt e.V. Tel +49 (0)30 - 3087748- 0
Panoramastr 1 Fax +49 (0)30 – 3087748 - 29
10178 Berlin Mail info@ibu-epd.com
Germany Web www.ibu-epd.com
Author of the Life Cycle
Assessment Tel +39 0544 467132
thinkstep Italy Fax +39 0544 501464
Via Bovini 43 Mail info@thinkstep.com
48123 Ravenna Web www.thinkstep.com
Italy
Owner of the Declaration
Isolparma srl Tel 049 9126213
Piazza Luigi da Porto 14 Fax 049 9129616
35131 Padova Mail info@isolparma.it
Italy Web www.isolparma.it
