ENVIRONMENTAL-PRODUCT DECLARATION
as per ISO 14025 and EN 15804+A2
Owner of the Declaration Kingspan Insulation B.V.
Publisher Institut Bauen und Umwelt e.V. (IBU)
Programme holder Institut Bauen und Umwelt e.V. (IBU)
Declaration number EPD-KIN-20230015-CBD2-EN
Issue date 07.02.2023
Valid to 06.02.2028
Therma™ TW50 / Therma™ TW50 EUR
Kingspan Insulation B.V.
www.ibu-epd.com | https://epd-online.com
General Information
Kingspan Insulation B.V. Therma™ TW50 / Therma™ TW50 EUR
Programme holder Owner of the declaration
IBU – Institut Bauen und Umwelt e.V. Kingspan Insulation B.V.
Hegelplatz 1 Lingewei 8
10117 Berlin 4004LL Tiel
Germany Netherlands
Declaration number Declared product / declared unit
EPD-KIN-20230015-CBD2-EN Therma™ TW50 / Therma™ TW50 EUR
1m2, 120mm thickness, R = 5,45 m2.K/W
D
This declaration is based on the product category rules: Scope:
Insulating materials made of foam plastics, 08.03.2023 The insulation materials Therma™ TW50 and Therma™ TW50 EUR are
(PCR checked and approved by the SVR) produced by Kingspan Insulation at the manufacturing facilities in
Winterswijk (the Netherlands), Burkhardtsdorf (Germany) and Kankaanpää
(Finland). This EPD is based on
Issue date weighted averages which have been determined on
the basis of the single values originating from the different Kingspan
07.02.2023
Insulation factories.
Therma™ TW50 / Therma™ TW50 EUR Cavity Board is an insulation
board with a rigid thermoset
Valid to
polyisocyanurate (PIR) fibre-free insulation core, faced on both sides with
06.02.2028 a low
emissivity composite foil. Therma™ TW50 Cavity Board is used as thermal
insulation for cavity walls.
In order to enable the user of the EPD to calculate the LCA results for
different thicknesses, the EPD contains the respective calculation rules.
The owner of the declaration shall be liable for the underlying information
and evidence; the IBU shall not be liable with respect to manufacturer
information, life cycle assessment data and evidences.
The EPD was created according to the specifications of EN 15804+A2. In
the following, the standard will be simplified as EN 15804 bezeichnet.
Dipl.-Ing Hans Peters
Verification
(chairman of Institut Bauen und Umwelt e.V.)
The standard EN 15804 serves as the core PCR
Independent verification of the declaration and data according to ISO
14025:2011
internally X externally
Dr. Alexander Röder Vito D'Incognito,
(Managing Director Institut Bauen und Umwelt e.V.) (Independent verifier)
1 Environmental-Product Declaration - Kingspan Insulation B.V. - Therma™ TW50 / Therma™ TW50 EUR
Product
Performance data of the product in accordance with the
Product description/Product definition declaration of performance with respect to its essential
Therma™ TW50 / Therma™ TW50 EUR Cavity Board is an characteristics according to EN 13165 - Thermal insulation
insulation board with a rigid thermoset polyisocyanurate (PIR) products for buildings - Factory made rigid polyurethane foam
fibre-free insulation core, faced on both sides with a low (PU) products - Specification
emissivity composite foil. The products are available in variable The declaration of performance of the product can be found at
thicknesses from 20 mm up to 200 mm. This EPD is based on a www.kingspan.com.
thickness of 120 mm and R -value of 5,45 m²·K/W. For the
D
Base materials/Ancillary materials
placing on the market of the product in the European
Union/European Free Trade Association (EU/EFTA) (with the The product contains approximately 3,3 kg/m2 polyurethane
exception of Switzerland) Regulation (EU) No. 305/2011 (CPR) rigid foam and 0,3 kg/m2 multi-layer aluminium facings.
applies. The product needs a declaration of performance taking The main materials of the polyurethane foam are MDI (between
into consideration EN 13165 - Thermal insulation products for 57-62 %), polyol (between 27-32 %) and a blowing agent
buildings - Factory made polyurethane foam (PU) products - (between 5-6 %). Due to the closed-cell structure (conform EN
Specification and the CE-marking. For the application and use 13165), the blowing agent remains in the foam. Water, flame
the respective national provisions apply. retardants and additives are added (between 4-8 %).
Application In the current REACH regulations, polyurethane foam
Therma™ TW50 / Therma™ TW50 EUR Cavity Board is used insulation products are considered “articles” and are
as thermal insulation for cavity walls. exempt from the requirements of Articles 57 and 59(1)
of REACH Regulation (EC) No 1907/2006. These
Technical Data
products are not classified as “hazardous products”
The technical specifications of the products within the scope of according to any current legislation, and can hence be
the EPD shall be listed, including the reference to the test declared as follows:
methods/test standards for each specification. - This article contains substances listed in the
candidate list (date: 31.08.2022) exceeding 0.1
For products with CE marking, the technical specifications must
percentage by mass: no.
be specified in accordance with information in the declaration of
- This article contains other carcinogenic, mutagenic,
performance. The properties relevant to the product should be
reprotoxic (CMR) substances in categories 1A or 1B
specified in the table below. If no information is given for
which are not on the candidate list, exceeding 0.1
properties, an explanation must be given in the background
percentage by mass: no.
report to the EPD as to why the property is not relevant to the
- Biocide products were added to this construction
product.
product or it has been treated with biocide products
(this then concerns a treated product as defined by the
Constructional data (EU) Biocidal Products Regulation No. 528/2012
Name Value Unit (BPR): no.
Thermal conductivity according to EN 0.022 W/(m.K) Environment and health during use
13165
Reaction to fire according to EN 13165 for Reference service life
F
Therma™ TW50 The reference service life is not to be declared in this
Reaction to fire according to EN 13165 for EPD as it does not cover the use stage.
E
Therma™ TW50 EUR
Compressive strength according to EN CS(10\Y)
13165 100
Thickness tolerance according to EN
T2-T3
13165
LCA: Calculation rules
The scope of this EPD is the thermal insulation products
Declared Unit Therma™ TW50 and Therma™ TW50 EUR as produced by
The declared unit (1 m²) and conversion factors are Kingspan Insulation at the manufacturing facilities in
listed in the table below. Winterswijk (the Netherlands), Burkhardtsdorf (Germany) and
Declared unit Kankaanpää (Finland).
Name Value Unit
The environmental impacts have been calculated per plant over
Declared unit 1 m2 the calendar year 2021. Based on the one year production
Gross density 30 kg/m3 volume of Therma™ TW50 and Therma™ TW50 EUR per
Grammage 3.6 kg/m2 plant, the individual environmental impacts are weighted.
Layer thickness 0.12 m
The EPD is studied for a common product thickness of 120
This EPD is based on a weighted average of the annual mm. Multiplication factors are included to calculate impacts for
production volume of three factories producing the products other product thicknesses within the range of 20 to 200 mm.
Therma™ TW50 and Therma™ TW50 EUR.
2 Environmental-Product Declaration - Kingspan Insulation B.V. - Therma™ TW50 / Therma™ TW50 EUR
For IBU core EPDs (where clause 3.6 is part of the EPD): for
average EPDs, an estimate of the robustness of the LCA Environmental burden of the incineration (R1 > 60 %) of the
values must be made, e.g. concerning variability of the product
production process, geographical representativeness and the at the end-of-life stage are assigned to the product system
influence of background data and preliminary products (C3); resulting potential credits for thermal and electrical energy
compared to the environmental impacts caused by actual from energy substitution are declared in module D.
production.
Geographic Representativeness
Land or region, in which the declared product system is
System boundary manufactured, used or handled at the end of the product´s
The type of EPD according to EN 15804 is: lifespan: Europe
cradle to gate with options, modules C1–C4, and
module D (A1–A3, C, D and additional modules:
A4, A5). Comparability
Basically, a comparison or an evaluation of EPD data is only
The product stage is a mandatory information module and it possible if all the data sets to be compared were created
covers: according to EN 15804 and the building context, respectively
· A1, raw material extraction and processing, processing of the product-specific characteristics of performance, are taken
secondary material input (e.g. recycling processes), into account.
· A2, transport to the manufacturer,
· A3, manufacturing, including provision of all materials, Background database
products and energy, packaging processing and its transport, Background data from GaBi ts Version 10 is used with
as well as waste processing up to the end-of-waste state or GaBi data sets CUP2022.1.
disposal of final residues
during the product stage.
The construction process stage includes: Factors for different thicknesses
· A4 transport to the building site; The LCA results for the insulation material declared in this EPD
· A5 installation in the building including provision of all refer to a product with a thickness of 120 mm. To enable the
materials, products and energy, as well as waste processing up user of the EPD to calculate the results for different thicknesses
to the end-of- waste state or disposal of final residues during the factors in the following table can be used for the calculation.
the construction process stage. The LCA results in chapter 5 have to be multiplied by these
factors.
The end-of-life stage is a mandatory information module and it
covers: The scaling factors are applicable for the complete
· C1 de-construction, demolition; product, where the multi-layer aluminium facings are
· C2 transport to waste processing; for all product thicknesses equal and the foam inputs
· C3 waste processing for reuse, recovery and/or recycling; are scaling upwards and downwards with other product
· C4 disposal (not applicable for this EPD) including provision thicknesses.
and all transport, provision of all materials, products and related
energy and water use.
LCA: Scenarios and additional technical information
Characteristic product properties assessment.
Information on biogenic carbon
Manufacturing (A3)
The total mass of biogenic carbon containing materials is less A polyethylene packaging foil is used. The products
than 5 % of the total mass of the product and accompanying are transported either on expanded polystyrene (EPS) skids or
packaging. on wooden pallets.
Technical information Within Module A3 the following packaging of the final
The following technical information is a basis for the product is included:
declared modules or can be used for developing - Polyethylene cover and wrap: 0,052 kg/m²
specific scenarios in the context of a building - Expanded Polystyrene skid: 0,02 kg/m²
3 Environmental-Product Declaration - Kingspan Insulation B.V. - Therma™ TW50 / Therma™ TW50 EUR
- Wooden pallet: 0,0 kg/m² The same holds for a service life declared by the manufacturer.
Corresponding information related to in-use conditions needs
Transport to the building site (A4)
not be provided if a service life taken from the list on service life
Name Value Unit
by BNB is declared.
Litres of fuel 0.0103 l/100km
Transport distance 100 km
End of life (C1-C4)
Gross density of products transported 30 kg/m3 The assumptions for C1 are: diesel-driven excavator (100 kW;
0.2 litre fuel per ton excavated material). The assumptions for
Installation into the building (A5)
C2 are: Truck Euro 6, diesel driven, 26-28 t gross weight,
Name ValueUnit assumed distance 50 km
Total output substances following waste treatment Name Value Unit
0.072 kg
on-site packaging material
Collected as mixed construction waste 3.6 kg
The recycling of the packaging is considered in A5. Energy recovery 3.6 kg
Reuse, recovery and/or recycling potentials (D), relevant
scenario information
In case a reference service life according to applicable ISO
Waste incineration with energy recuperation is assumed as an
standards is declared then the assumptions and in-use
end-of-life scenario
conditions underlying the determined RSL shall be declared. In
addition, it shall be stated that the RSL applies for the reference
conditions only.
4 Environmental-Product Declaration - Kingspan Insulation B.V. - Therma™ TW50 / Therma™ TW50 EUR
LCA: Results
In Table 1 "Description of the system boundary", all declared modules shall be indicated with an "X"; all modules that are not declared
shall be indicated with "MND" (As default the modules B3, B4, B5 are marked as MNR – module not relevant). In the following tables,
columns can be deleted for modules that are not declared. Indicator values should be declared with three valid digits (eventually using
exponential form (e.g. 1,23E-5 = 0,0000123). A uniform format should be used for all values of one indicator.
If several modules are not declared and therefore have been deleted from the table, the abbreviations for the indicators can be
replaced by the complete names, while the readability and clear arrangement should be maintained; the legends can then be deleted.
If due to relevant data gaps, an indicator cannot be declared in a robust way, then the abbreviation “IND” (indicator not declared)
should be used for this indicator.
• 0 - calculated value is 0
• 0 - value falls under the cut-off
• 0 - assumption which exclude any flows (e.g. exported
electricity A1-A3)
• IND – in cases where the inventory does not support
the methodological approach or the calculation of the
specific indicator IND shall be used.
If no reference service life is declared (see chapter 2.13 "Reference Service Life"), the LCA results of the modules B1-B2 and B6-B7
shall refer to a period of one year. This shall then be indicated as an explanatory text below the tables. In addition, the formula for the
quantification of such B-modules over the total life cycle shall be provided.
DESCRIPTION OF THE SYSTEM BOUNDARY (X = INCLUDED IN LCA; ND = MODULE OR INDICATOR NOT DECLARED; MNR =
MODULE NOT RELEVANT)
BENEFITS
AND LOADS
CONSTRUCTION
BEYOND
PRODUCT STAGE PROCESS USE STAGE END OF LIFE STAGE
THE SYSTEM
STAGE
BOUNDARIE
S
la ire ta m w a Ry lp p u s tro p s n a rT g n iru tc a fu n a M e h t m o rf tro p s n a rTe tis e h t o t e ta g y lb m e s s A e s U e c n a n e tn ia M ria p e R tn e m e c a lp e R tn e m h s ib ru fe R y g re n e la n o ita re p Oe s u re ta w la n o ita re p Oe s u n o itc u rts n o c -e Dn o itilo m e d tro p s n a rT g n is s e c o rp e ts a W la s o p s iD -e s u e R-y re v o c e R-g n ilc y c e Rla itn e to p
A1 A2 A3 A4 A5 B1 B2 B3 B4 B5 B6 B7 C1 C2 C3 C4 D
X X X X X MND MND MNR MNR MNR MND MND X X X X X
RESULTS OF THE LCA - ENVIRONMENTAL IMPACT according to EN 15804+A2: 1m2 120mm Therma™ TW50 / Therma™
TW50 EUR
Parameter Unit A1-A3 A4 A5 C1 C2 C3 C4 D
GWP-total kg CO 2-Äq. 9.85E+00 3.03E-02 1.8E-01 2.31E-03 1.51E-02 7.79E+00 0 -3.2E+00
GWP-fossil kg CO 2-Äq. 1.01E+01 3.02E-02 1.8E-01 2.31E-03 1.51E-02 7.63E+00 0 -3.18E+00
GWP-biogenic kg CO 2-Äq. -2.37E-01 -4.17E-05 9.84E-06 3.09E-06 -2.08E-05 1.66E-01 0 -1.58E-02
GWP-luluc kg CO 2-Äq. 6.64E-03 1.68E-04 2.14E-06 2.85E-08 8.41E-05 1.43E-05 0 -3.63E-04
ODP kg CFC11-Äq. 2.89E-11 1.81E-15 3.21E-14 1.41E-16 9.04E-16 5.77E-13 0 -2.04E-11
AP mol H+-Äq. 2.15E-02 3.11E-05 2.25E-05 1.07E-05 1.55E-05 4.55E-03 0 -4.89E-03
EP-freshwater kg PO 4-Äq. 4.57E-05 9.01E-08 8.1E-09 4.65E-10 4.5E-08 1.56E-07 0 -4.2E-06
EP-marine kg N-Äq. 5.5E-03 1.02E-05 6.02E-06 5.1E-06 5.09E-06 2.2E-03 0 -1.18E-03
EP-terrestrial mol N-Äq. 5.67E-02 1.21E-04 1.02E-04 5.59E-05 6.06E-05 2.53E-02 0 -1.27E-02
kg NMVOC-
POCP 2.72E-02 2.74E-05 1.74E-05 1.45E-05 1.37E-05 5.64E-03 0 -3.34E-03
Äq.
ADPE kg Sb-Äq. 1.17E-05 2.52E-09 7.83E-10 9.44E-11 1.26E-09 1.58E-08 0 -4.65E-07
ADPF MJ 2.64E+02 4.03E-01 6.65E-02 3.12E-02 2.02E-01 2.02E+00 0 -5.33E+01
m3 world-Äq.
WDP 1.54E+00 2.71E-04 1.71E-02 4.29E-06 1.35E-04 7.72E-01 0 -3.5E-01
deprived
GWP = Global warming potential; ODP = Depletion potential of the stratospheric ozone layer; AP = Acidification potential of land and water; EP =
Eutrophication potential; POCP = Formation potential of tropospheric ozone photochemical oxidants; ADPE = Abiotic depletion potential for non-fossil
resources; ADPF = Abiotic depletion potential for fossil resources; WDP = Water (user) deprivation potential)
RESULTS OF THE LCA - INDICATORS TO DESCRIBE RESOURCE USE according to EN 15804+A2: 1m2 120mm Therma™
TW50 / Therma™ TW50 EUR
Parameter Unit A1-A3 A4 A5 C1 C2 C3 C4 D
PERE MJ 2.97E+01 2.29E-02 1.71E-02 1.18E-04 1.15E-02 3.54E-01 0 -1.52E+01
PERM MJ 0 0 0 0 0 0 0 0
PERT MJ 2.97E+01 2.29E-02 1.71E-02 1.18E-04 1.15E-02 3.54E-01 0 -1.52E+01
PENRE MJ 1.5E+02 4.04E-01 3.11E+00 3.13E-02 2.02E-01 1.13E+02 0 -5.33E+01
5 Environmental-Product Declaration - Kingspan Insulation B.V. - Therma™ TW50 / Therma™ TW50 EUR
PENRM MJ 1.14E+02 0 -3.04E+00 0 0 -1.11E+02 0 0
PENRT MJ 2.64E+02 4.04E-01 6.65E-02 3.13E-02 2.02E-01 2.02E+00 0 -5.33E+01
SM kg 0 0 0 0 0 0 0 0
RSF MJ 0 0 0 0 0 0 0 0
NRSF MJ 0 0 0 0 0 0 0 0
FW m3 7.08E-02 2.59E-05 4.06E-04 1.78E-07 1.3E-05 1.82E-02 0 -1.64E-02
PERE = Use of renewable primary energy excluding renewable primary energy resources used as raw materials; PERM = Use of renewable primary
energy resources used as raw materials; PERT = Total use of renewable primary energy resources; PENRE = Use of non-renewable primary energy
excluding non-renewable primary energy resources used as raw materials; PENRM = Use of non-renewable primary energy resources used as raw
materials; PENRT = Total use of non-renewable primary energy resources; SM = Use of secondary material; RSF = Use of renewable secondary fuels;
NRSF = Use of non-renewable secondary fuels; FW = Use of net fresh water
RESULTS OF THE LCA – WASTE CATEGORIES AND OUTPUT FLOWS according to EN 15804+A2:
1m2 120mm Therma™ TW50 / Therma™ TW50 EUR
Parameter Unit A1-A3 A4 A5 C1 C2 C3 C4 D
HWD kg 1.12E-07 1.94E-12 5.54E-12 1.03E-13 9.68E-13 2.76E-10 0 -6.59E-09
NHWD kg 2.85E-01 5.79E-05 1.62E-02 2.93E-06 2.9E-05 4.37E-02 0 -8.03E-02
RWD kg 2.75E-03 4.98E-07 2.77E-06 3.43E-08 2.49E-07 8.4E-05 0 -4.17E-03
CRU kg 0 0 0 0 0 0 0 0
MFR kg 0 0 0 0 0 2.54E-02 0 0
MER kg 0 0 7.21E-02 0 0 3.46E+00 0 0
EEE MJ 0 0 3.27E-01 0 0 1.32E+01 0 0
EET MJ 0 0 5.85E-01 0 0 2.36E+01 0 0
HWD = Hazardous waste disposed; NHWD = Non-hazardous waste disposed; RWD = Radioactive waste disposed; CRU = Components for re-use;
MFR = Materials for recycling; MER = Materials for energy recovery; EEE = Exported electrical energy; EET = Exported thermal energy
RESULTS OF THE LCA – additional impact categories according to EN 15804+A2-optional:
1m2 120mm Therma™ TW50 / Therma™ TW50 EUR
Parameter Unit A1-A3 A4 A5 C1 C2 C3 C4 D
Disease
PM 1.81E-07 1.8E-10 2.74E-10 1.21E-10 8.98E-11 1.27E-08 0 -4.26E-08
incidence
IR kBq U235-Äq. 3.34E-01 7.3E-05 3.8E-04 4.99E-06 3.65E-05 1.35E-02 0 -7.12E-01
ETP-fw CTUe 1.08E+02 2.8E-01 4.76E-02 2.17E-02 1.4E-01 6.96E-01 0 -1.21E+01
HTP-c CTUh 7.3E-09 5.64E-12 2.67E-12 4.02E-13 2.82E-12 5.21E-11 0 -6.27E-10
HTP-nc CTUh 6.22E-07 2.93E-10 2.7E-10 2.03E-11 1.46E-10 1.9E-09 0 -2.21E-08
SQP SQP 6.35E+01 1.39E-01 1.7E-02 8.61E-05 6.94E-02 4.26E-01 0 -9.18E+00
PM = Potential incidence of disease due to PM emissions; IR = Potential Human exposure efficiency relative to U235; ETP-fw = Potential comparative
Toxic Unit for ecosystems; HTP-c = Potential comparative Toxic Unit for humans (cancerogenic); HTP-nc = Potential comparative Toxic Unit for humans
(not cancerogenic); SQP = Potential soil quality index
Disclaimer 1 – for the indicator “Potential Human exposure efficiency relative to U235”.This impact category deals mainly with the
eventual impact of low-dose ionizing radiation on human health of the nuclear fuel cycle. It does not consider effects due to possible
nuclear accidents, occupational exposure or to radioactive waste disposal in underground facilities. Potential ionizing radiation from the
soil, radon and from some construction materials is also not measured by this indicator.
Disclaimer 2 – for the indicators “abiotic depletion potential for non-fossil resources”, “abiotic depletion potential for fossil resources”,
“water (user) deprivation potential, deprivation-weighted water consumption”, “potential comparative toxic unit for ecosystems”,
“potential comparative toxic unit for humans – cancerogenic”, “Potential comparative toxic unit for humans - not cancerogenic”,
“potential soil quality index”. The results of this environmental impact indicator shall be used with care as the uncertainties on these
results are high as there is limited experience with the indicator.
References
Biocidal Products Regulation No. 528/2012 (BPR) EN 13165:2012+A2:2016: Thermal insulation products
Regulation (EU) No 528/2012 of the European for buildings. Factory made polyurethane foam (PU)
Parliament and of the Council of 22 May 2012 products. Specification
concerning the making available on the market and
use of biocidal products EN 15804
EN 15804:2012+A2:2019+AC:2021, Sustainability of
CPR construction works — Environmental Product
Regulation (EU) No. 305/2011 of the European Declarations — Core rules for the product category of
Parliament and of the Council of 9 March 2011 laying construction products.
down harmonised condition for the marketing of
construction products and repealing Council Directive GaBi ts
89/106/EC thinkstep AG: Leinfelden-Echterdingen GaBi Software-
System and Database for Life Cycle Engineering 1992-
ISO 14025 2019
EN ISO 14025:2011, Environmental labels and
declarations — Type III environmental declarations — IBU 2021
Principles and procedures. Institut Bauen und Umwelt e.V.: General Instructions
for the EPD programme of Institut Bauen und Umwelt
EN 13165 e.V., Version 2.0, Berlin: Institut Bauen und Umwelt
6 Environmental-Product Declaration - Kingspan Insulation B.V. - Therma™ TW50 / Therma™ TW50 EUR
e.V., 2021. range of Environmental Product Declarations of Institut
www.ibu-epd.com Bauen und Umwelt (IBU), Part B: Requirements on the
EPD for insulating materials made of foam
LCA-tool plastics. January 2019
Kingspan LCA tool, version 1.1. IBU-KSI-202001-LT1-
EN. REACH
Developed by Sphera Solutions GmbH (formely Regulation (EC) No 1907/2006 of the European
Thinkstep GmbH) Parliament and of the Council on the Registration,
Evaluation, Authorisation and Restriction of Chemicals
PCR Version 1.7, Part A (REACH)
Institut Bauen und Umwelt e.V., Berlin (pub.): Product https://echa.europa.eu/candidate-list-table;
Category Rules for Building-Related Products and
services, Part A: Calculation Rules for the Life Cycle Candidate list
Assessment and Requirements on the Project Report https://echa.europa.eu/candidate-list-table; accessed
according to EN 15804+A2:2019 31.08.2022, 233 substances listed.
November 2021 The literature referred to in the Environmental Product
Declaration must be listed in full.Standards already fully quoted
PCR 2017, Part B in the EPD do not need to be listed here again.
Institut Bauen und Umwelt e.V., Berlin (pub.): Product The current version of PCR Part A and PCR Part B of the PCR
Category Rules for Construction Products from the document on which they are based must be referenced.
7 Environmental-Product Declaration - Kingspan Insulation B.V. - Therma™ TW50 / Therma™ TW50 EUR
Publisher
Institut Bauen und Umwelt e.V. +49 (0)30 3087748- 0
Hegelplatz 1 info@ibu-epd.com
10117 Berlin www.ibu-epd.com
Germany
Programme holder
Institut Bauen und Umwelt e.V. +49 (0)30 3087748- 0
Hegelplatz 1 info@ibu-epd.com
10117 Berlin www.ibu-epd.com
Germany
Author of the Life Cycle Assessment
Kingspan Insulation B.V. +31 (0) 543 543 210
Lingewei 8 info@kingspaninsulation.nl
4004LL Tiel www.kingspan.com
Netherlands
Owner of the Declaration
Kingspan Insulation B.V. +31 (0) 543 543 210
Lingewei 8 info@kingspaninsulation.nl
4004LL Tiel www.kingspan.com
Netherlands
8 Environmental-Product Declaration - Kingspan Insulation B.V. - Therma™ TW50 / Therma™ TW50 EUR
