ENVIRONMENTAL PRODUCT DECLARATION
as per ISO 14025 and EN 15804+A2
Owner of the Declaration Kingspan Insulation B.V.
Publisher Institut Bauen und Umwelt e.V. (IBU)
Programme holder Institut Bauen und Umwelt e.V. (IBU)
Declaration number EPD-KSI-20230320-CBA1-EN
Issue date 22.09.2023
Valid to 21.09.2028
Kooltherm® K12 D
Kingspan Insulation B.V.
www.ibu-epd.com | https://epd-online.com
General Information
Kingspan Insulation B.V. Kooltherm® K12 D
Programme holder Owner of the declaration
IBU – Institut Bauen und Umwelt e.V. Kingspan Insulation B.V.
Hegelplatz 1 Lingewei 8
10117 Berlin 4004LL Tiel
Germany Netherlands
Declaration number Declared product / declared unit
EPD-KSI-20230320-CBA1-EN Kooltherm® K12 D Framing Board
1 m², 100 mm thickness, R = 4,75 m²·K/W
D
This declaration is based on the product category rules: Scope:
Insulating materials made of foam plastics, 01.08.2021 The insulation material Kooltherm® K12 D, is produced by Kingspan
(PCR checked and approved by the SVR) Insulation B.V. at the manufacturing facilities in Tiel, the Netherlands and
Jönköping, Sweden. This EPD is based on weighted averages which have
been determined on the basis of the single values originating from the
Issue date different Kingspan Insulation factories.
22.09.2023
Kooltherm® K12 D is a rigid thermoset cellular insulation material faced on
both sides with a micro-perforated aluminum foil.
Valid to
In order to enable the user of the EPD to calculate the LCA results for
21.09.2028 different thicknesses, the EPD contains the respective calculation rules.
The owner of the declaration shall be liable for the underlying information
and evidence; the IBU shall not be liable with respect to manufacturer
information, life cycle assessment data and evidences.
The EPD was created according to the specifications of EN 15804+A2. In
the following, the standard will be simplified as EN 15804.
Verification
The standard EN 15804 serves as the core PCR
Dipl.-Ing. Hans Peters Independent verification of the declaration and data according to ISO
(Chairman of Institut Bauen und Umwelt e.V.) 14025:2011
internally X externally
Florian Pronold Vito D'Incognito,
(Managing Director Institut Bauen und Umwelt e.V.) (Independent verifier)
1 Environmental Product Declaration - Kingspan Insulation B.V. - Kooltherm® K12 D
Product
products for buildings - Factory made phenolic foam (PF)
Product description/Product definition products - Specification
Kooltherm® K12 D is a rigid thermoset cellular insulation
material faced on both sides with a composite foil based facing. Base materials/Ancillary materials
The product is available in variable thicknesses from 40 mm up The main materials are phenolic (PF) resin (between 70-80%)
to 120 mm. This EPD is based on a thickness of 100 mm and with added catalyst and additives (between 15-20%). Phenolic
R -value of 4,75 m²·K/W. rigid foam onto a facing material (between 5-10%) is formed by
D
the chemical reaction of these materials and adding a blowing
agent with no ozone depletion potential (ca. 5%). Due to the
For the placing on the market of the product in the European
closed-cell structure (conform EN 13166), the blowing agent
Union/European Free Trade Association (EU/EFTA) (with the
remains in the foam.
exception of Switzerland) Regulation (EU) No. 305/2011 (CPR)
applies. The product needs a declaration of performance taking
In the current REACH regulations, phenolic foam insulation
into consideration EN 13166 - Thermal insulation products for
products are considered 'articles' and are exempt from the
buildings - Factory made phenolic foam (PF) products -
requirements of Article 57 and 59(1) of REACH Regulation (EC)
specification and the CE-marking. For the application and use
No 1907/2006. These products are not classified as 'hazardous
the respective national provisions apply.
products' according to any current legislation, and can hence
Application be declared as follows:
Kooltherm® K12 D is suitable for use as insulation for framing
systems. - This article contains substances listed in the candidate list
(date: 17.01.2023) exceeding 0.1 percentage by mass: no.
Technical Data - This article contains other carcinogenic, mutagenic, reprotoxic
The declaration of performance of the product can be found at (CMR) substances in categories 1A or 1B which are not on the
www.kingspan.com. candidate list, exceeding 0.1 percentage by mass: no.
- Biocide products were added to this construction product or it
Constructional data
has been treated with biocide products (this then concerns a
Name Value Unit treated product as defined by the (EU) Biocidal Products
Compressive strength acc. to EN 13166 ≥ 100 kPa Regulation No. 528/2012 (BPR): no.
Thermal conductivity λd acc. to EN 13166 0.021 W/(mK)
The chemical functional group of the additives used in the resin
Technical parameters not included are modulus of elasticity as
is that of non-ionic surfactants.
well as sound absorption (not relevant for this application) and
creep (not placed under permanent load). Reference service life
The reference service life is not to be declared in this EPD as it
Performance data of the product in accordance with the
does not cover the use stage.
declaration of performance with respect to its essential
characteristics according to EN 13166- Thermal insulation
LCA: Calculation rules
Declared Unit System boundary
The declared unit (1 m²) and conversion factors are listed in the Type of EPD: according to EN 15804: cradle to gate with
table below. options, modules C1–C4, and module D (A1–A3, C, D and
additional modules: A4,A5).
Declared unit
Name Value Unit
The product stage is a mandatory information module and it
Declared unit 1 m2 covers:
Gross density (foam) 35 kg/m3 · A1, raw material extraction and processing, processing of
secondary material input (e.g. recycling processes),
Grammage 3.735 kg/m2
· A2, transport to the manufacturer,
Layer thickness 0.1 m
· A3, manufacturing, including provision of all materials,
This EPD is based on a weighted average of the annual products and energy, packaging processing and its transport,
production volume of two factories producing the products as well as waste processing up to the end-of-waste state or
Kooltherm® K12 D. The scope of this EPD is the thermal disposal of final residues during the product stage.
insulation product Kooltherm® K12 D as produced by Kingspan
The construction process stage includes:
Insulation at the manufacturing facilities in Tiel (the
· A4 transport to the building site;
Netherlands), and Jönköping (Sweden). The environmental
· A5 installation in the building including provision of all
impacts have been calculated per plant over the calendar year
2022. Based on the one-year production volume of Kooltherm® materials, products and energy, as well as waste processing up
to the end-of-waste state or disposal of final residues during the
K12 D per plant, the individual environmental impacts are
construction process stage.
weighted.
The end-of-life stage is a mandatory information module and it
The EPD is studied for a common product thickness of 100mm.
covers:
Multiplication factors are included to calculate impacts for other
· C1 de-construction, demolition;
product thicknesses within the range of 20 to 120 mm.
· C2 transport to waste processing;
2 Environmental Product Declaration - Kingspan Insulation B.V. - Kooltherm® K12 D
· C3 waste processing for reuse, recovery and/or recycling; Environmental burden of the incineration (R1 > 60%) of the
· C4 disposal (not applicable for this EPD) including provision product at the end-of-life stage are assigned to the product
and all transport, provision of all materials, products and related system (C3); resulting potential credits for thermal and electrical
energy and water use. energy from energy substitution are declared in module D.
data sets CUP2022.1
Factors for different thicknesses
The LCA results for the insulation material declared in this EPD
refer to a product with a thickness of 100 mm. To enable the Geographic Representativeness
user of the EPD to calculate the results for different thicknesses Land or region, in which the declared product system is
the factors in the following table can be used for the calculation. manufactured, used or handled at the end of the product´s
The LCA results in chapter 5 have to be multiplied by these lifespan: Europe
factors. The scaling factors are applicable for the complete
product, where the facings are for all product thicknesses
Comparability
equal, and the foam inputs are scaling upwards and
Basically, a comparison or an evaluation of EPD data is only
downwards with other product thicknesses.
possible if all the data sets to be compared were created
according to EN 15804 and the building context, respectively
the product-specific characteristics of performance, are taken
into account.
Background data from GaBi ts Version 10 is used with GaBi
LCA: Scenarios and additional technical information
Installation into the building (A5)
Characteristic product properties of biogenic carbon
The total mass of biogenic carbon containing materials is less Name ValueUnit
than 5 % of the total mass of the product and accompanying Output substances following waste treatment on
0.06 kg
packaging. site packaging material
Technical information
The recycling of the packaging is considered in A5.
The following technical information is a basis for the declared
modules or can be used for developing specific scenarios in the
context of a building assessment. End of life (C1-C4)
The assumptions for C1 are: diesel driven excavator (100 kW;
Manufacturing (A3) 0.2 litre fuel per ton excavated material).
Within A1-A3 the following packaging of the final product is The assumptions for C2 are: Truck Euro 6, diesel driven, 26-28
included: t gross weight, assumed distance 50 km
Polyethylene cover and wrap: 0,05 kg/m² Name Value Unit
Others (mainly Expanded Polystyrene skid): 0,01 kg/m²
Collected as mixed construction waste 3.735 kg
Energy recovery 3.735 kg
Transport to the building site (A4)
R1-value of waste incineration plant >60 %
Name Value Unit
Litres of fuel 0.0103 l/100km
Reuse, recovery and/or recycling potentials (D), relevant
Transport distance 100 km scenario information
Grammage of products transproted 3.735 kg/m² Waste incineration with energy recuperation is assumed as
end-of-life scenario.
3 Environmental Product Declaration - Kingspan Insulation B.V. - Kooltherm® K12 D
LCA: Results
DESCRIPTION OF THE SYSTEM BOUNDARY (X = INCLUDED IN LCA; ND = MODULE OR INDICATOR NOT DECLARED; MNR =
MODULE NOT RELEVANT)
Benefits and
Construction loads beyond
Product stage Use stage End of life stage
process stage the system
boundaries
la ire ta m w a Ry lp p u s tro p s n a rT g n iru tc a fu n a M e h t m o rf tro p s n a rTe tis e h t o t e ta g y lb m e s s A e s U e c n a n e tn ia M ria p e R tn e m e c a lp e R tn e m h s ib ru fe R y g re n e la n o ita re p Oe s u re ta w la n o ita re p Oe s u n o itc u rts n o c -e Dn o itilo m e d tro p s n a rT g n is s e c o rp e ts a W la s o p s iD -e s u e R-y re v o c e R-g n ilc y c e Rla itn e to p
A1 A2 A3 A4 A5 B1 B2 B3 B4 B5 B6 B7 C1 C2 C3 C4 D
X X X X X MND MND MNR MNR MNR MND MND X X X X X
RESULTS OF THE LCA - ENVIRONMENTAL IMPACT according to EN 15804+A2: 1 m2 100 mm thickness
Parameter Unit A1-A3 A4 A5 C1 C2 C3 C4 D
GWP-total kg CO 2 eq 7.46E+00 3.14E-02 1.88E-01 2.4E-03 1.57E-02 8.03E+00 0 -3.88E+00
GWP-fossil kg CO 2 eq 7.63E+00 3.13E-02 1.88E-01 2.39E-03 1.57E-02 8.03E+00 0 -3.86E+00
GWP-biogenic kg CO 2 eq -2.44E-01 -4.32E-05 1.03E-05 3.2E-06 -2.16E-05 5.46E-04 0 -1.79E-02
GWP-luluc kg CO 2 eq 8.02E-02 1.75E-04 2.23E-06 2.95E-08 8.73E-05 1.43E-05 0 -4.75E-04
ODP kg CFC11 eq 1.42E-08 1.88E-15 3.35E-14 1.47E-16 9.38E-16 5.88E-13 0 -2.18E-11
AP mol H+ eq 1.65E-02 3.23E-05 2.34E-05 1.11E-05 1.61E-05 4.74E-03 0 -7.78E-03
EP-freshwater kg P eq 2.57E-05 9.35E-08 8.46E-09 4.83E-10 4.67E-08 1.58E-07 0 -4.62E-06
EP-marine kg N eq 4.43E-03 1.06E-05 6.29E-06 5.29E-06 5.28E-06 2.29E-03 0 -1.55E-03
EP-terrestrial mol N eq 4.4E-02 1.26E-04 1.07E-04 5.8E-05 6.28E-05 2.64E-02 0 -1.67E-02
kg NMVOC
POCP 2.25E-02 2.84E-05 1.81E-05 1.5E-05 1.42E-05 5.89E-03 0 -4.48E-03
eq
ADPE kg Sb eq 7.22E-06 2.62E-09 8.18E-10 9.79E-11 1.31E-09 1.62E-08 0 -5.25E-07
ADPF MJ 2.1E+02 4.18E-01 6.94E-02 3.24E-02 2.09E-01 2.07E+00 0 -6.25E+01
m3 world eq
WDP 1.2E+00 2.81E-04 1.78E-02 4.45E-06 1.4E-04 7.91E-01 0 -4.5E-01
deprived
GWP = Global warming potential; ODP = Depletion potential of the stratospheric ozone layer; AP = Acidification potential of land and water; EP =
Eutrophication potential; POCP = Formation potential of tropospheric ozone photochemical oxidants; ADPE = Abiotic depletion potential for non-fossil
resources; ADPF = Abiotic depletion potential for fossil resources; WDP = Water (user) deprivation potential)
RESULTS OF THE LCA - INDICATORS TO DESCRIBE RESOURCE USE according to EN 15804+A2: 1 m2 100 mm thickness
Parameter Unit A1-A3 A4 A5 C1 C2 C3 C4 D
PERE MJ 3.4E+01 2.38E-02 1.78E-02 1.22E-04 1.19E-02 3.61E-01 0 -1.91E+01
PERM MJ 0 0 0 0 0 0 0 0
PERT MJ 3.4E+01 2.38E-02 1.78E-02 1.22E-04 1.19E-02 3.61E-01 0 -1.91E+01
PENRE MJ 1.05E+02 4.19E-01 3.27E+00 3.24E-02 2.1E-01 1.04E+02 0 -6.25E+01
PENRM MJ 1.05E+02 0 -3.21E+00 0 0 -1.02E+02 0 0
PENRT MJ 2.1E+02 4.19E-01 6.95E-02 3.24E-02 2.1E-01 2.07E+00 0 -6.25E+01
SM kg 0 0 0 0 0 0 0 0
RSF MJ 0 0 0 0 0 0 0 0
NRSF MJ 0 0 0 0 0 0 0 0
FW m3 5.56E-02 2.69E-05 4.24E-04 1.84E-07 1.35E-05 1.86E-02 0 -2.53E-02
PERE = Use of renewable primary energy excluding renewable primary energy resources used as raw materials; PERM = Use of renewable primary
energy resources used as raw materials; PERT = Total use of renewable primary energy resources; PENRE = Use of non-renewable primary energy
excluding non-renewable primary energy resources used as raw materials; PENRM = Use of non-renewable primary energy resources used as raw
materials; PENRT = Total use of non-renewable primary energy resources; SM = Use of secondary material; RSF = Use of renewable secondary fuels;
NRSF = Use of non-renewable secondary fuels; FW = Use of net fresh water
RESULTS OF THE LCA – WASTE CATEGORIES AND OUTPUT FLOWS according to EN 15804+A2:
1 m2 100 mm thickness
Parameter Unit A1-A3 A4 A5 C1 C2 C3 C4 D
HWD kg 9.57E-05 2.01E-12 5.79E-12 1.07E-13 1E-12 2.85E-10 0 -6.09E-09
NHWD kg 3.3E-01 6.01E-05 1.69E-02 3.04E-06 3.01E-05 4.04E-02 0 -2.36E-01
RWD kg 2.81E-03 5.17E-07 2.89E-06 3.56E-08 2.58E-07 8.55E-05 0 -4.78E-03
CRU kg 0 0 0 0 0 0 0 0
MFR kg 0 0 0 0 0 9.72E-02 0 0
MER kg 0 0 7.53E-02 0 0 3.64E+00 0 0
EEE MJ 0 0 3.42E-01 0 0 1.39E+01 0 0
EET MJ 0 0 6.11E-01 0 0 2.48E+01 0 0
HWD = Hazardous waste disposed; NHWD = Non-hazardous waste disposed; RWD = Radioactive waste disposed; CRU = Components for re-use;
MFR = Materials for recycling; MER = Materials for energy recovery; EEE = Exported electrical energy; EET = Exported thermal energy
4 Environmental Product Declaration - Kingspan Insulation B.V. - Kooltherm® K12 D
RESULTS OF THE LCA – additional impact categories according to EN 15804+A2-optional:
1 m2 100 mm thickness
Parameter Unit A1-A3 A4 A5 C1 C2 C3 C4 D
Disease
PM 1.79E-07 1.86E-10 2.86E-10 1.26E-10 9.31E-11 1.31E-08 0 -7.23E-08
incidence
IR kBq U235 eq 4.66E-01 7.57E-05 3.97E-04 5.18E-06 3.79E-05 1.37E-02 0 -8.33E-01
ETP-fw CTUe 7.86E+01 2.91E-01 4.97E-02 2.25E-02 1.45E-01 7.07E-01 0 -1.5E+01
HTP-c CTUh 3.19E-09 5.86E-12 2.79E-12 4.17E-13 2.93E-12 5.34E-11 0 -9.74E-10
HTP-nc CTUh 1.16E-07 3.04E-10 2.82E-10 2.11E-11 1.52E-10 1.94E-09 0 -2.96E-08
SQP SQP 3.93E+01 1.44E-01 1.77E-02 8.93E-05 7.2E-02 4.34E-01 0 -9.86E+00
PM = Potential incidence of disease due to PM emissions; IR = Potential Human exposure efficiency relative to U235; ETP-fw = Potential comparative
Toxic Unit for ecosystems; HTP-c = Potential comparative Toxic Unit for humans (cancerogenic); HTP-nc = Potential comparative Toxic Unit for humans
(not cancerogenic); SQP = Potential soil quality index
Disclaimer 1 – for the indicator IR
This impact category deals mainly with the eventual impact of low dose ionizing radiation on human health of the nuclear fuel cycle. It
does not consider effects due to possible nuclear accidents, occupational exposure nor due to radioactive waste disposal in
underground facilities. Potential ionizing radiation from the soil, from radon and from some construction materials is also not measured
by this indicator.
Disclaimer 2 – for the indicators ADPE, ADPF, WDP, ETP-fw, HTP-c, HTP-nc, SQP
The results of this environmental impact indicator shall be used with care as the uncertainties on these results are high or as there is
limited experienced with the indicator. This EPD was created using a software tool.
References
EN 13166 ISO 14025
EN 13166:2012+A2:2016: Thermal insulation products for EN ISO 14025:2011-10 - Environmental labels and declarations
buildings. Factory made phenolic foam (PF) products. — Type III environmental declarations — Principles and
Specification procedures
EN 15804+A2 LCA-tool
EN15804/A2: Sustainability of construction works - Kingspan LCA tool, version 1.2. IBU-KSI-202001-LT1-EN.
Environmental product declarations - Core rules for the product Developed by Sphera Solutions GmbH (formely Thinkstep
category of construction products, 2019 GmbH)
BPR PCR Version 1.7, Part A
Regulation (EU) No 528/2012 of the European Parliament and Institut Bauen und Umwelt e.V., Berlin (pub.): Product Category
of the Council of 22 May 2012 concerning the making available Rules for Building-Related Products andservices, Part A:
on the market and use of biocidal products Calculation Rules for the Life Cycle Assessment and
Requirements on the Project Report according to EN
15804+A2:2019 November 2021
CPR
Regulation (EU) No. 305/2011 of the European Parliament and
of the Council of 9 March 2011 laying down harmonised PCR, Part B
condition for the marketing of construction products and Institut Bauen und Umwelt e.V., Berlin (pub.): Product Category
repealing Council Directive 89/106/EC Rules for Construction Products from the range of
Environmental Product Declarations of Institut Bauen und
Umwelt (IBU), Part B: Requirements on the EPD for insulating
GaBi ts materials made of foam plastics. June 2023
thinkstep AG: Leinfelden-Echterdingen GaBi Software-System
and Database for Life Cycle Engineering 1992-2019 REACH
Regulation (EC) No 1907/2006 of the European Parliament and
of the Council on the Registration, Evaluation, Authorisation
IBU 2021 and Restriction of Chemicals (REACH)
Institut Bauen und Umwelt e.V.: General Instructions for the https://echa.europa.eu/candidate-list-table; accessed 17th of
EPD programme of Institut Bauen und Umwelte.V., Version 2.0, January 2023, 233 substances listed.
Berlin: Institut Bauen und Umwelte.V., 2021. www.ibu-epd.com
5 Environmental Product Declaration - Kingspan Insulation B.V. - Kooltherm® K12 D
Publisher
Institut Bauen und Umwelt e.V. +49 (0)30 3087748- 0
Hegelplatz 1 info@ibu-epd.com
10117 Berlin www.ibu-epd.com
Germany
Programme holder
Institut Bauen und Umwelt e.V. +49 (0)30 3087748- 0
Hegelplatz 1 info@ibu-epd.com
10117 Berlin www.ibu-epd.com
Germany
Author of the Life Cycle Assessment
Kingspan Insulation B.V. +31 (0) 543 543 210
Lingewei 8 info@kingspaninsulation.nl
4004LL Tiel www.kingspan.com
Netherlands
Owner of the Declaration
Kingspan Insulation B.V. +31 (0) 543 543 210
Lingewei 8 info@kingspaninsulation.nl
4004LL Tiel www.kingspan.com
Netherlands
6 Environmental Product Declaration - Kingspan Insulation B.V. - Kooltherm® K12 D
