ENVIRONMENTAL PRODUCT DECLARATION
as per ISO 14025 and EN 15804+A2
Owner of the Declaration Shaw Contract (Shaw Europe Ltd.)
Publisher Institut Bauen und Umwelt e.V. (IBU)
Programme holder Institut Bauen und Umwelt e.V. (IBU)
Declaration number EPD-SHA-20220301-CCA3-EN
Issue date 19/09/2023
Valid to 18/09/2028
TaskWorx® Carpet Tile with EcoSolution Q100™ Face Fibre
Shaw Contract (Shaw Europe Ltd.)
www.ibu-epd.com | https://epd-online.com
General Information
Shaw Contract (Shaw Europe Ltd.) TaskWorx® Carpet Tile with EcoSolution Q100™
Face Fibre
Programme holder Owner of the declaration
IBU – Institut Bauen und Umwelt e.V. Shaw Contract (Shaw Europe Ltd.)
Hegelplatz 1 Blackaddie Road *
10117 Berlin DG46DB Sanquhar
Germany United Kingdom
Declaration number Declared product / declared unit
EPD-SHA-20220301-CCA3-EN 1 m2 of installed TaskWorx® Carpet Tile
This declaration is based on the product category rules: Scope:
Floor coverings, 01/08/2021 A Life Cycle Assessment (LCA) was conducted based upon production
(PCR checked and approved by the SVR) data collected from Shaw Contract (Shaw Europe, Ltd.), Plant SQ
manufacturing facility (Blackaddie Road, Sanquhar, DG46DB), located in
Scotland, UK. Production data was collected for TaskWorx® Carpet Tile
Issue date with EcoSolution Q100™ Face Fibre, for the period of one year, from
January to December 2021.
19/09/2023
This EPD is cradle-to-gate with options in scope with additional modules
A4, A5, B1 and B2. The EPD is created in accordance to the specifications
of EN 15804+A2.
Valid to
18/09/2028 The functional unit has been defined as 1m2 of installed TaskWorx® Carpet
Tile.
The EPD was generated with the help of an LCA Tool, version 1.
The owner of the declaration shall be liable for the underlying information
and evidence; the IBU shall not be liable with respect to manufacturer
information, life cycle assessment data and evidences.
The EPD was created according to the specifications of EN 15804+A2. In
the following, the standard will be simplified as EN 15804.
Dipl.-Ing. Hans Peters Verification
(Chairman of Institut Bauen und Umwelt e.V.)
The standard EN 15804 serves as the core PCR
Independent verification of the declaration and data according to ISO
14025:2011
internally X externally
Florian Pronold Mrs Kim Allbury,
(Managing Director Institut Bauen und Umwelt e.V.) (Independent verifier)
1 Environmental Product Declaration - Shaw Contract (Shaw Europe Ltd.) - TaskWorx® Carpet Tile with EcoSolution Q100™ Face Fibre
Product
Constructional data
Product description/Product definition
This EPD covers all products which comprise the TaskWorx® Name Value Unit
collection and which feature the TaskWorx® backing system Product Form Carpet Tile -
together with EcoSolution Q100TM Nylon face fibre. Yarn type - Solution-dyed 100% Post-industrial
-
Nylon 6 Recycled Content
TaskWorx® is a commercial carpet tile, for use as a floor Total thickness 6 - 8 mm
covering in accordance with the manufacturer's guidelines. Total carpet weight 4094 - 5163 g/m2
Surface pile thickness 1.2 - 3.4 mm
The carpet tile consists of Shaw's unique face fibre, Nylon 6,
Surface pile weight -
manufactured with 100% recycled material on the TaskWorx® 576 - 949 g/m2
Nominal Pile Mass
backing system, a modified bitumen
Length and width of squared
compound with 100% natural recycled mineral filler, and a 250 - 1000 mm
elements
fibreglass reinforcement layer.
Other technical data parameters listed in IBU PCR Part B are
The EcoSolution Q100TM face fibre is tufted into a primary not relevant and, therefore, have not been declared.
backing sheet containing recycled content. Latex is added to
anchor the fibre and the TaskWorx® backing system is then Performance data of the product in accordance with the
applied. declaration of performance with respect to its essential
characteristics according to 14041:2004A/C:2006.
TaskWorx® is suitable for use in all commercial settings. It has
Base materials/Ancillary materials
a life span of 15
years, and it comes with a 15-year warranty (subject only to TaskWorx® Carpet Tile with EcoSolution Q100™ Face Fibre is
installation and maintenance being carried out in line with comprised of the following raw materials:
manufacturer's guidelines). • 40-60% Calcium Carbonate, containing Recycled
Content
The product meets both internal and external performance • 18-20% Modified Bitumen Polymer
standards including those established in the EU under EN 1307 • 15-18% Solution Dyed Nylon 6 Face Fibre, containing
and EN 10874 for a product suitable for heavy and general 100% Post-industrial Recycled Content
commercial installations. • 3-5% Styrene Butadiene Co-Polymer Latex
• 2-5% Polyester Primary & Secondary Backing
At the end of product life, the Shaw Contract take back • 0.5-2% Fibreglass Reinforcement
recycling scheme: re[TURN]® is available for this product. • 0-0.25% Anti-stat
Details may be obtained at www.shawcontract.com. The product is packaged in cardboard boxes, wrapped in
For the placing on the market of the product in the European plastic, and stacked on wooden pallets for distribution.
Union/European Free Trade Association (EU/EFTA) (with the
exception of Switzerland) Regulation (EU) No. 305/2011 (CPR) This product contains substances listed in the candidate list
applies. The product needs a declaration of performance taking (date: 17.01.2023) exceeding 0.1 percentage by mass: no.
into consideration EN 14041:2004A/C:2006, and the CE-
marking. This product contains other CMR substances in categories 1A
or 1B which are not on the candidate list, exceeding 0.1
For the application and use the respective national provisions percentage by mass: no
apply.
Biocide products were added to this construction product or it
Application
has been treated with biocide products (this then concerns a
TaskWorx® Carpet Tile with EcoSolution Q100™ Face Fibre is treated product as defined by the (EU) Ordinance on Biocide
suitable for use as a floor covering in heavy and general Products No. 528/2012): no
commercial installations.
Reference service life
Technical Data When properly installed as a commercial floor covering,
The technical specifications of the product are listed on the TaskWorx® with EcoSolution Q100™ face fibre has a reference
product's specification sheet, found at www.shawcontract.com. service life of 15 years. This carpet tile product comes with a
This product meets the requirements of the harmonized 15-year warranty, subject only to installation and maintenance
European Norm (hEN): EN14041:2004A/C:2006. Declarations being carried out in accordance with the manufacturer's
of performance related to fire, electrostatic, formaldehyde guidelines.
emissions, and slip resistance can be found on the product's
specification sheet.
LCA: Calculation rules
Name Value Unit
Declared Unit
Declared unit 1 m2
The declaration refers to the declared unit of 1 m² of installed
carpet tile. Grammage 4.292 kg/m2
Layer thickness 0.007 m
Declared unit
2 Environmental Product Declaration - Shaw Contract (Shaw Europe Ltd.) - TaskWorx® Carpet Tile with EcoSolution Q100™ Face Fibre
End-of-Life Stage:
System boundary Three scenarios have been evaluated:
The type of EPD is Cradle-to-Gate with options modules C1– Scenario 1: the TaskWorx® carpet is 100% disposed of in a
C4, module D, and additional modules. The additional modules landfill.
are A4, A5, B1 and B2. Scenario 2: the TaskWorx® carpet is 100% incinerated.
Scenario 3: 40% of TaskWorx® carpets are incinerated and the
The modules considered in the life cycle assessment and remaining 60% are landfilled. This assumption is based on the
environmental product declaration, based on the product's carpet disposal rates in Europe mentioned in the study
entire life cycle, are described as follows: conducted by Deutsche Umwelthilfe in 2017 (Umwelthilfe,
2017) and the European Commission in 2013 (Comission,
Production Stage: 2013).
• Module A1 - Provision of Raw Materials. • Module C1 - The carpet is de-constructed manually and
• Module A2 - Transport of Raw Materials. no
• Module A3 - Manufacturing. additional environmental impact is caused.
Construction/Installation Stage: • Module C2 - Transport of the carpet waste to a landfill or
• Module A4 - Transportation by truck of the product to the to the
construction site in Europe. municipal waste incineration plant.
• Module A5 - Installation of the carpet, treatment of • Module C3 - Impacts from thermal treatment disposal
cutting waste (landfill) and packaging waste (landfill, (C3/2 and C3/3).
recycling, and incineration). The production of the • Module C4 - Impacts from landfill disposal (C4/1 and
amount of carpet that occurs as installation waste is C4/3).
also included along with its transport to the place of Module D includes benefits from energy recovery via treatment
installation. of packaging materials and incineration of carpets at their end
Biogenic carbon that is stored in the wooden pallets and of life (D/1, D/2 and D/3), as well as the burdens of balancing
cardboard (packaging) is released as carbon dioxide the secondary material content in modules A1 and A3 via the
emissions into the air at the end of life in module A5. net-scrap approach.
Use Stage:
Geographic Representativeness
• Module B1 - Indoor emissions of volatile organic Land or region, in which the declared product system is
compounds (VOCs) during the first few months after manufactured, used or handled at the end of the product´s
installation. lifespan: Europe
• Module B2 - Carpet cleaning per year, including
vacuuming (electricity consumption) and hot water
cleaning (electricity and water consumption, as well as Comparability
waste water treatment). Basically, a comparison or an evaluation of EPD data is only
• Module B3 - Repair (module not relevant). possible if all the data sets to be compared were created
• Module B4 - Replacement (module not relevant). according to EN 15804 and the building context, respectively
• Module B5 - Refurbishment (module not relevant). the product-specific characteristics of performance, are taken
• Module B6 - Operational Energy Use (module not into account. The used background database used for the
relevant). creation of the EPD : GaBi ts software, CUP 2022.2.
• Module B7 - Operational Water Use (module not
relevant).
LCA: Scenarios and additional technical information
installation of TaskWorx® carpet tile and should be used in
Characteristic product properties of biogenic carbon
accordance with the manufacturer's guidelines. Installation
Biogenic carbon is only present in packaging (wooden pallets losses have been accounted for in module A5. Product losses
and cardboards). Assumed water content in wooden pallet are considered as 5%.
(packaging): 18%.
Information on describing the Biogenic Carbon Content at The packaging material treatment and disposal are also
factory gate considered in module A5 (landfill, recycling, and incineration)
and the resulting benefits from energy generation are included
Name ValueUnit
in module D. The quantity of wooden pallets used is 0.133 kg
Biogenic carbon content in accompanying kg
0.14 per m². Wooden pallets are assumed to be re-used 20 times
packaging C
before being disposed of. Hence, the quantity of pallet disposed
is 0.007 kg. The quantity of cardboard packaging is 0.21 kg/m²
The following technical scenario information is required for the and the quantity of plastic packaging is 0.0103 kg/m². Total
declared modules and optional for non-declared modules. amount of packaging disposed at installation is 0.227 kg.
Packaging disposal rates (Source: Eurostat, Recovery and
Transport to the construction site (A4)
recycling rates for packaging).
Name Value Unit
• Paper - 82.8% recycled; 9.4% landfilled; and 7.8%
Transport distance (truck) 687 km
incinerated
Capacity utilisation (including empty runs) 55 %
• Plastic - 40.3% recycled; 28.7% landfilled; and 31.0%
incinerated
Installation in the building (A5)
• Wood pallets - 39.8% recycled; 34.5% landfilled; and
The installation of TaskWorx® is done manually and no energy 25.7% incinerated
is required. A Pressure-Sensitive adhesive is required for the
3 Environmental Product Declaration - Shaw Contract (Shaw Europe Ltd.) - TaskWorx® Carpet Tile with EcoSolution Q100™ Face Fibre
Name ValueUnit End of Life (C1-C4)
Auxiliary (adhesive) 0.23 kg C1 - The product dismantling from the building is done
Material loss (5% cutting losses) 0.215 kg manually without energy burden.
Output substances following waste treatment on C2 - Transportation of the product to the end of life is assumed
0.227 kg
site (packaging materials) to be 161 km (100 miles).
C3/2: The TaskWorx carpet is 100% combusted in and
Use (B1) see cap. 2.12 use incineration plant with energy recovery (R>0.6).
Name Value Unit
C3/3: It is assumed that 40% of TaskWorx carpets are
Emissons to air (TVOC) after 50 days - Indoor Air
900 mg/m² incinerated and the remaining 60% are landfilled.
Comfort Gold®
Emission testing was conducted in accordance to Eurofins C4/1: The TaskWorx carpet product is 100% disposed of in a
Indoor Air Comfort Gold® certification. After 28 days, the landfill.
specific concentration of TVOCs was < 100 ug/m3, as required C4/3: It is assumed that 40% of TaskWorx carpets are
by the certification standard. incinerated and the remaining 60% are landfilled.
Name ValueUnit
Maintenance (B2) Collected as mixed construction waste 4.292 kg
For the maintenance of TaskWorx® Carpet Tile, 2 hot water Landfilling (Scenario 1 - C3/1, C4/1 and D/1) 4.292 kg
extraction cleanings (water and electricity consumption) per Incineration (Scenario 2 - C3/2, C4/2, and D/2) 4.292 kg
year as well as 52 vacuum cleanings (electricity consumption)
Landfilling (60%) and Incineration (40%) (Scenario
per year are recommended. The Reference Service Life of the 4.292 kg
3 - C3/3, C4/3 and D/3)
product is 15 years. The results in the EPD declare a
maintenance for the period of 1 year.
Reuse, recovery and/or recycling potentials (D), relevant
Name Value Unit
scenario information
Water consumption (1 year) 0.0009 m3
Electricity consumption (1 year) 0.772 kWh For the thermal and electrical energy generated in Module A5
due to thermal treatment of packaging, avoided burdens have
been calculated by the inversion of electricity grid mix and
Reference service life thermal energy from natural gas, using European datasets.
Name ValueUnit
Reference service life (according to ISO 15686-1, - Module D also includes the environmental burdens linked to the
15 a
2, -7 and -8) supply to secondary materials (nylon and calcium carbonate)
used in the carpet production.
Life Span according to the manufacturer 15 a
4 Environmental Product Declaration - Shaw Contract (Shaw Europe Ltd.) - TaskWorx® Carpet Tile with EcoSolution Q100™ Face Fibre
LCA: Results
The B2 module declares the maintenance (cleaning) per one year. The user of the EPD will be able to scale the results for its entire
useful life by multiplying the impact by the RSL.
Three end of life scenarios were considered in the EPD.
Scenario 1: TaskWorx carpet is 100% landfilled. (C3/1, C4/1 and D/1).
Scenario 2: TaskWorx carpet is 100% incinerated with energy recovery (R>0.6) (C3/2, C4/2 and D/2).
Scenario 3: 40% of TaskWorx carpets are incinerated and the remaining 60% are landfilled (C3/3, C4/3 and D/3).
DESCRIPTION OF THE SYSTEM BOUNDARY (X = INCLUDED IN LCA; ND = MODULE OR INDICATOR NOT DECLARED; MNR =
MODULE NOT RELEVANT)
Benefits and
Construction loads beyond
Product stage Use stage End of life stage
process stage the system
boundaries
la ire ta m w a Ry lp p u s tro p s n a rT g n iru tc a fu n a M e h t m o rf tro p s n a rTe tis e h t o t e ta g y lb m e s s A e s U e c n a n e tn ia M ria p e R tn e m e c a lp e R tn e m h s ib ru fe R y g re n e la n o ita re p Oe s u re ta w la n o ita re p Oe s u n o itc u rts n o c -e Dn o itilo m e d tro p s n a rT g n is s e c o rp e ts a W la s o p s iD -e s u e R-y re v o c e R-g n ilc y c e Rla itn e to p
A1 A2 A3 A4 A5 B1 B2 B3 B4 B5 B6 B7 C1 C2 C3 C4 D
X X X X X X X MNR MNR MNR MND MND X X X X X
RESULTS OF THE LCA - ENVIRONMENTAL IMPACT according to EN 15804+A2: 1 m² TaskWorx® Carpet
Parameter Unit A1-A3 A4 A5 B1 B2 C1 C2 C3/1 C3/2 C3/3 C4/1 C4/2 C4/3 D/1 D/2 D/3
GWP-total kg CO 2 3.46E 2.68E-01 2.85E- 2.54E- 2.89E- 0 5.81E- 0 4.75E 1.9E+003.01E-01 0 1.81E-01 5.22E 3.93E 4.71E
eq +00 01 04 01 02 +00 +00 +00 +00
GWP-fossil kg CO 2 3.8E+00 2.67E-01 2.44E- 2.54E- 2.86E- 0 5.79E- 0 4.74E 1.9E+003.04E-01 0 1.83E-015.2E+00 3.92E 4.69E
eq 01 04 01 02 +00 +00 +00
GWP- kg CO 2 -3.41E- -3.68E- 4.09E- 0 3.05E- 0 -8E-05 0 2.64E- 1.06E- -3.24E- 0 -1.94E- 2.13E- 1.09E-02 1.71E-
biogenic eq 01 04 02 03 03 03 03 03 02 02
GWP-luluc kg CO 2 1.87E-031.49E-03 1.91E- 0 6.06E- 0 3.23E- 0 1.26E- 5.05E- 1.48E-04 0 8.89E-05 3.77E- 1.36E-04 2.81E-
eq 04 05 04 04 05 04 04
kg CFC11 4.36E- 4.19E- 3.47E- 2.82E- 1.13E- 8.44E- -7.96E- 1.88E-
ODP 8.28E-09 1.6E-14 0 0 0 4.09E-13 0 2.45E-13
eq 10 12 15 12 12 12 12 12
mol H+ 6.27E- 6.29E- 5.97E- 1.83E- 9.61E- 8.59E-
AP 1.04E-022.75E-04 0 0 0 7.3E-04 9.02E-04 0 5.41E-04 7.06E-03
eq 04 04 05 03 03 03
EP- 4.38E- 1.73E- 3.52E- 4.26E- 2.95E-
kg P eq 2.15E-057.96E-07 0 1.4E-06 0 0 8.8E-07 5.68E-05 0 3.41E-05 9.85E-07
freshwater 06 07 07 06 06
1.55E- 1.43E- 1.95E- 2.48E- 2.71E- 2.47E-
EP-marine kg N eq 2.48E-038.99E-05 0 0 0 6.2E-04 1.99E-04 0 1.2E-04 2.12E-03
04 04 05 04 03 03
1.66E- 1.48E- 2.32E- 8.58E- 3.43E- 2.33E- 2.08E-
EP-terrestrial mol N eq 2.68E-021.07E-03 0 0 0 2.19E-03 0 1.31E-03 1.71E-02
03 03 04 03 03 02 02
kg
5.06E- 1.41E- 3.82E- 5.26E- 1.64E- 6.55E- 8.74E-
POCP NMVOC 8.21E-032.42E-04 0 0 6.42E-04 0 3.85E-04 7.13E-03 8.1E-03
04 05 04 05 03 04 03
eq
3.38E- 4.84E- 4.59E- 1.84E- 5.42E- 4.17E-
ADPE kg Sb eq 5.9E-07 2.23E-08 0 7.8E-08 0 0 2.11E-08 0 1.27E-08 2.29E-07
08 09 08 08 07 07
9.52E 3.56E 5.49E 5.19E 7.74E- 4.88E 1.95E 4.32E 2.59E 1.05E 8.17E 9.55E
ADPF MJ 0 0 0 0
+01 +00 +00 +00 01 +00 +00 +00 +00 +02 +01 +01
m3 world
2.66E- 6.54E- 5.19E- 7.64E- 3.06E- 2.06E- -5.04E- 1.03E-
WDP eq 4.24E-012.39E-03 0 0 0 -3E-03 0 -1.8E-03
02 02 04 01 01 01 02 01
deprived
GWP = Global warming potential; ODP = Depletion potential of the stratospheric ozone layer; AP = Acidification potential of land and water; EP =
Eutrophication potential; POCP = Formation potential of tropospheric ozone photochemical oxidants; ADPE = Abiotic depletion potential for non-fossil
resources; ADPF = Abiotic depletion potential for fossil resources; WDP = Water (user) deprivation potential)
RESULTS OF THE LCA - INDICATORS TO DESCRIBE RESOURCE USE according to EN 15804+A2: 1 m² TaskWorx® Carpet
Parameter Unit A1-A3 A4 A5 B1 B2 C1 C2 C3/1 C3/2 C3/3 C4/1 C4/2 C4/3 D/1 D/2 D/3
1.13E 2.13E- 4.22E 2.88E 1.81E 7.22E- 3.55E- 2.13E- -7.19E -4.15E-
PERE MJ 0 0 4.4E-02 0 0 4.1E+00
+01 01 +00 +00 +00 01 01 01 +00 01
5.31E -4.19E
PERM MJ 0 0 0 0 0 0 0 0 0 0 0 0 0 0
+00 +00
1.66E 2.13E- 2.88E 1.81E 7.22E- 3.55E- 2.13E- -7.19E -4.15E-
PERT MJ 3.01E-02 0 0 4.4E-02 0 0 4.1E+00
+01 01 +00 +00 01 01 01 +00 01
4.18E 3.76E 5.19E 7.76E- 6.29E 2.52E 4.32E 2.59E 1.05E 8.18E 9.56E
PENRE MJ 6.1E-01 0 0 0 0
+01 +00 +00 01 +01 +01 +00 +00 +02 +01 +01
5.84E -3.17E- -5.8E -2.32E
PENRM MJ 0 0 0 0 0 0 0 0 0 0 0 0
+01 01 +01 +01
9.87E 3.76E 5.19E 7.76E- 4.89E 1.95E 4.32E 2.59E 1.05E 8.18E 9.56E
PENRT MJ 2.94E-01 0 0 0 0
+01 +00 +00 01 +00 +00 +00 +00 +02 +01 +01
5 Environmental Product Declaration - Shaw Contract (Shaw Europe Ltd.) - TaskWorx® Carpet Tile with EcoSolution Q100™ Face Fibre
3.03E -3.19E -3.19E -3.19E
SM kg 0 1.6E-01 0 0 0 0 0 0 0 0 0 0
+00 +00 +00 +00
RSF MJ 0 0 0 0 0 0 0 0 0 0 0 0 0 0 0 0
NRSF MJ 0 0 0 0 0 0 0 0 0 0 0 0 0 0 0 0
1.84E- 2.29E- 2.75E- 4.98E- 1.77E- 7.09E- 5.59E- 3.35E- 1.05E- -3.02E-
FW m3 1.09E-03 0 0 0 0 6.17E-03
02 04 03 05 02 03 05 05 02 04
PERE = Use of renewable primary energy excluding renewable primary energy resources used as raw materials; PERM = Use of renewable primary
energy resources used as raw materials; PERT = Total use of renewable primary energy resources; PENRE = Use of non-renewable primary energy
excluding non-renewable primary energy resources used as raw materials; PENRM = Use of non-renewable primary energy resources used as raw
materials; PENRT = Total use of non-renewable primary energy resources; SM = Use of secondary material; RSF = Use of renewable secondary fuels;
NRSF = Use of non-renewable secondary fuels; FW = Use of net fresh water
RESULTS OF THE LCA – WASTE CATEGORIES AND OUTPUT FLOWS according to EN 15804+A2:
1 m² TaskWorx® Carpet
Parameter Unit A1-A3 A4 A5 B1 B2 C1 C2 C3/1 C3/2 C3/3 C4/1 C4/2 C4/3 D/1 D/2 D/3
8.38E- 1.71E- 4.41E- 4.49E- 3.72E- 4.64E- 1.86E- 6.66E- 3.99E- 9.43E-
HWD kg 0 0 0 0 7.18E-09 8.53E-09
07 11 08 10 12 10 10 10 10 09
3.96E- 5.12E- 2.66E- 4.77E- 1.11E- 4.22E- 1.69E- 4.27E 2.56E 5.44E- -1.06E- -9.59E-
NHWD kg 0 0 0 0
01 04 01 03 04 01 01 +00 +00 03 02 04
3.96E- 2.14E- 9.56E- 3.21E- 1.29E- 3.18E- 7.04E- -2.55E- -5.96E-
RWD kg 4.4E-06 0 8.3E-04 0 0 5.3E-05 0
03 04 07 04 04 05 04 03 04
CRU kg 0 0 0 0 0 0 0 0 0 0 0 0 0 0 0 0
1.81E-
MFR kg 0 0 0 0 0 0 0 0 0 0 0 0 0 0 0
01
MER kg 0 0 0 0 0 0 0 0 0 0 0 0 0 0 0 0
6.37E- 1.09E 4.37E
EEE MJ 0 0 0 0 0 0 0 0 0 0 0 0 0
02 +01 +00
9.77E- 2.35E 9.39E-
EET MJ 0 0 0 0 0 0 0 0 0 0 0 0 0
02 +00 01
HWD = Hazardous waste disposed; NHWD = Non-hazardous waste disposed; RWD = Radioactive waste disposed; CRU = Components for re-use;
MFR = Materials for recycling; MER = Materials for energy recovery; EEE = Exported electrical energy; EET = Exported thermal energy
RESULTS OF THE LCA – additional impact categories according to EN 15804+A2-optional:
1 m² TaskWorx® Carpet
Parameter Unit A1-A3 A4 A5 B1 B2 C1 C2 C3/1 C3/2 C3/3 C4/1 C4/2 C4/3 D/1 D/2 D/3
Disease 1.21E- 1.59E- 7.08E- 5.21E- 3.45E- 2.36E- 9.42E- 8.66E- 7.58E-
PM 0 0 0 0 5.2E-09 5.46E-086.73E-08
incidence 07 09 09 09 10 08 09 09 08
kBq U235 4.18E- 6.45E- 2.29E- 1.41E- 1.32E- 7.83E- 1.09E- -4.41E- -1.11E-
IR 0 0 1.4E-04 0 3.3E-02 0 4.7E-03
eq 01 04 02 01 02 03 01 01 01
2.47E 5.17E- 2.35E 5.37E- 4.22E 2.53E 4.54E
ETP-fw CTUe 5.7E+01 3.4E+00 0 0 2.1E+00 8.4E-01 0 4.9E+01 4E+01
+00 04 +00 01 +00 +00 +01
1.58E- 4.99E- 9.76E- 6.79E- 1.08E- 3.32E- 1.14E- 1.39E-
HTP-c CTUh 0 0 0 8.3E-11 1.9E-10 0 1.11E-091.28E-09
09 11 11 11 11 11 10 09
9.46E- 2.59E- 6.12E- 3.73E- 2.65E- 5.62E- 4.76E- 1.91E- 1.59E- 9.54E- 5.27E-
HTP-nc CTUh 0 0 0 4.25E-084.86E-08
08 09 09 12 09 10 09 09 08 09 08
1.22E 1.23E 7.38E- 1.87E 2.66E- 1.47E 5.86E- 3.11E- 1.86E- 2.43E -4.91E -5.06E-
SQP SQP 0 0 0 0
+01 +00 01 +00 01 +00 01 01 01 +00 +00 01
PM = Potential incidence of disease due to PM emissions; IR = Potential Human exposure efficiency relative to U235; ETP-fw = Potential comparative
Toxic Unit for ecosystems; HTP-c = Potential comparative Toxic Unit for humans (cancerogenic); HTP-nc = Potential comparative Toxic Unit for humans
(not cancerogenic); SQP = Potential soil quality index
Disclaimer 1 – for the indicator 'Potential Human exposure efficiency relative to U235'. This impact category deals mainly with the
eventual impact of low dose ionizing radiation on human health of the nuclear fuel cycle. It does not consider effects due to possible
nuclear accidents, occupational exposure nor due to radioactive waste disposal in underground facilities. Potential ionizing radiation
from the soil, from radon and from some construction materials is also not measured by this indicator.
Disclaimer 2 – for the indicators 'abiotic depletion potential for non-fossil resources', 'abiotic depletion potential for fossil resources',
'water (user) deprivation potential, deprivation-weighted water consumption', 'potential comparative toxic unit for ecosystems', 'potential
comparative toxic unit for humans – carcinogenic', 'Potential comparative toxic unit for humans - not carcinogenic', 'potential soil quality
index'. The results of this environmental impact indicator shall be used with care as the uncertainties on these results are high or as
there is limited experienced with the indicator. This EPD was created using a software tool.
References
STANDARDS: EN 14041:2004/AC:2006 — Resilient, textile and laminate floor
coverings — Essential characteristics.
EN 10874
EN 10874:2009, Resilient, textile and laminate floor coverings EN 15804
— Classification. EN 15804:2012+A2:2019/AC:2021, Sustainability of
construction works — Environmental product declarations —
EN 1307 Core rules for the product category of construction products.
EN 1307:2014, Textile floor coverings — Classification.
ISO 14025
EN 14041 ISO 14025:2011, Environmental labels and declarations —
6 Environmental Product Declaration - Shaw Contract (Shaw Europe Ltd.) - TaskWorx® Carpet Tile with EcoSolution Q100™ Face Fibre
Type III environmental declarations — Principles and Problem of the Carpet Industry in Germany, 2017.
procedures.
GaBi
ISO 14040 GaBi Software System and Database for Life Cycle
ISO 14040:2006, Environmental management — Life cycle Engineering, 1992-2021, Sphera Solutions GmbH, Leinfelden-
assessment — Principles and framework. Echterdingen, with acknowledgement of LBP University of
Stuttgart, program version GaBi 10; database version 2021.1.
ISO 14044
ISO 14044:2006, Environmental management — Life cycle GaBi documentation
assessment — Requirements and guidelines. GaBi dataset documentation for the software system and
databases, LBP, University of Stuttgart and Sphera Solutions
ISO 15686 GmbH, Leinfelden-Echterdingen, 2021 (http://www.gabi-
ISO 15686-1:2011, Building and constructed assets — Service software.com/support/gabi/gabi-database-2021-lci-
life planning — Part 1: General principles and framework. documentation/).
ISO 15686 IBU 2021
ISO 15686-2:2011, Building and constructed assets — Service Institut Bauen und Umwelt e.V.: General Instructions for the
life planning — Part 2: Service life prediction procedures. EPD programme of Institut Bauen und Umwelt e.V., Version
2.0,
ISO 15686 Berlin: Institut Bauen und Umwelt e.V., 2021 (www.ibu-
ISO 15686-7:2011, Building and constructed assets — Service epd.com).
life planning — Part 7: Performance evaluation for feedback of
service life data from practice. PCR Part A
PCR Part A: Calculation rules for the Life Cycle Assessment
ISO 15686 and Requirements on the Background Report according to EN
ISO 15686-8:2011, Building and constructed assets — Service 15804:2012+A2:2019/AC:2021, Version 1.3, Institut Bauen und
life planning — Part 8: Reference service life and service life Umwelt e.V., 2021.
estimation.
PCR Part B
FURTHER REFERENCES: Product Category Rules for Building Products, Part B:
Requirements on the EPD for floor coverings, version 1.7, 2022
Candidate list (www.bau-umwelt.de).
Candidate List of substances of very high concern for
Authorisation, published on ECHA website, latest version Packaging disposal rates
17.01.2023 (https://echa.europa.eu/candidatelist-table). Eurostat, Recovery and recycling rates for packaging. 2015
(http://ec.europa.eu/eurostat/web/environment/waste/main-
Deutsche Umwelthilfe tables).
Deutsche Umwelthilfe. Swept under the Carpet: The Big Waste
7 Environmental Product Declaration - Shaw Contract (Shaw Europe Ltd.) - TaskWorx® Carpet Tile with EcoSolution Q100™ Face Fibre
Publisher
Institut Bauen und Umwelt e.V. +49 (0)30 3087748- 0
Hegelplatz 1 info@ibu-epd.com
10117 Berlin www.ibu-epd.com
Germany
Programme holder
Institut Bauen und Umwelt e.V. +49 (0)30 3087748- 0
Hegelplatz 1 info@ibu-epd.com
10117 Berlin www.ibu-epd.com
Germany
Author of the Life Cycle Assessment
Sphera Solutions, Inc. +1 (312) 796-7160
130 East Randolph St 1900 info@sphera.com
60601 Chicago 130 E. Randolph St., Suite 2900
United States
Owner of the Declaration
Shaw Contract (Shaw Europe Ltd.) +1 800 257 7429
Blackaddie Road * infouk@shawcontract.com
DG46DB Sanquhar www.shawcontract.com
United Kingdom
8 Environmental Product Declaration - Shaw Contract (Shaw Europe Ltd.) - TaskWorx® Carpet Tile with EcoSolution Q100™ Face Fibre
