ENVIRONMENTAL PRODUCT DECLARATION
as per ISO 14025 and EN 15804+A2
Owner of the Declaration IVPU - Industrieverband Polyurethan-Hartschaum e.V.
Publisher Institut Bauen und Umwelt e.V. (IBU)
Programme holder Institut Bauen und Umwelt e.V. (IBU)
Declaration number EPD-IVP-20240424-IBE1-EN
Issue date 29.11.2024
Valid to 28.11.2029
PU thermal insulation boards with multi-layer aluminium facing
IVPU e.V.
www.ibu-epd.com | https://epd-online.com
1. General Information
IVPU e.V. PU thermal insulation boards with multi-layer
aluminium facing
Programme holder Owner of the declaration
IBU – Institut Bauen und Umwelt e.V. IVPU ­ Industrieverband Polyurethan­Hartschaum e.V.
Hegelplatz 1 Heilbronner Str. 154
10117 Berlin 70191 Stuttgart
Germany Germany
Declaration number Declared product / declared unit
EPD­IVP­20240424­IBE1­EN 1 m² of installed PU thermal insulation board with multi­layer aluminium
facing (on both sides), a thickness of 12 cm, and a nominal thermal
conductivity of 0.022 W/(m.K) and a delcared value of thermal resistance
of Rd = 5.45 (m²•K)/W.
This declaration is based on the product category rules: Scope:
Insulating materials made of foam plastics, 01.08.2021 This EPD applies to all declared products of the IVPU's member
(PCR checked and approved by the SVR) companies Karl Bachl GmbH & Co KG, Holcim Solution and Products
EMEA BV, IKO Insulation BV, Kingspan Insulation GmbH & Co KG,
Linzmeier Bauelemente GmbH, puren gmbh, Recticel NV/SA, Soprema
Issue date GmbH, Steinbacher Dämmstoff GmbH, Unilin Insulation bv. The IVPU
represents more than 90% of the companies within the German
29.11.2024
polyurethane insulation products market. This EPD is based on weighted
averages which have been determined on the basis of the single values
originating from the factories of the mentioned manufacturing companies
Valid to
(see section 3.1).
28.11.2029 The owner of the declaration shall be liable for the underlying information
and evidence; the IBU shall not be liable with respect to manufacturer
information, life cycle assessment data and evidences.
The EPD was created according to the specifications of EN 15804+A2. In
the following, the standard will be simplified as EN 15804.
Verification
The standard EN 15804 serves as the core PCR
Independent verification of the declaration and data according to ISO
14025:2011
Dipl.­Ing. Hans Peters internally X externally
(Chairman of Institut Bauen und Umwelt e.V.)
Florian Pronold Prof. Dr. Birgit Grahl,
(Managing Director Institut Bauen und Umwelt e.V.) (Independent verifier)
1 Environmental Product Declaration ­ IVPU e.V. ­ PU thermal insulation boards with multi­layer aluminium facing
2. Product
Name Value Unit
2.1 Product description/Product definition
Gross density 31 ­ 32 kg/m3
Factory made rigid polyurethane foam (PU) products are used
for the thermal insulation of buildings. PU includes both PIR Compressive stress at 10 %
and PUR products. The products are manufactured in the form deformation or strength acc. to EN 100 – 150 kPa
of boards without or with flexible facings. 826
This Product Declaration covers PU insulation boards with Tensile strength acc. to EN 1607 ≥ 40 kPa
multi­layer aluminium foil facings on both sides. For the placing Modulus of elasticity acc. to EN 826 ≥ 4 N/mm2
on the market of the product in the European Union/European
Calculation value for thermal
Free Trade Association (EU/EFTA) (with the exception of 0.023 W/(mK)
conductivity
Switzerland) Regulation (EU) No. 305/2011 (CPR) applies.
Water vapour diffusion resistance
The product needs a declaration of performance taking into ∞ ­
factor acc. to EN 12088
consideration EN 13165:2016-09 Thermal insulation products
for buildings ­ Factory made rigid polyurethane foam (PU) Dimensional stability under defined
DS(70/90)3 and
products ­ Specification and the CE­marking. temperature and humidity Class
DS(­20,­)1
For the design und execution of buidlings the respective conditions DS(TH)i
Member State's legislation applies. In Germany, the relevant Thermal conductivity acc. to EN
0.022 W/(mK)
requirements for insulation products are included in DIN 4108­ 13165
10. The design value of thermal conductivity is specified in DIN Limiting dimensions of thickness Ti T2 Class
4108­4.
Creep behaviour or permanent
compressive strength acc. to EN ≥ 0.02 N/mm2
2.2 Application
1606
The scope of application of PU rigid foam insulation materials
Declared value of thermal
includes thermal insulation in building construction (e.g. pitched 5.45 (m²•K)/W
resistance RD
roofs, flat roofs, floors, ceilings and exterior walls (inside and
outside). Thickness at RD = 1 (m²•K)/W 22 mm
Performance data of the production in accordance with the
2.3 Technical Data
declaration of performance with respect to its essential
For determining technical data, testing methods as stated in EN
characteristics according to DIN 4108-10: 2021-11 (Table 6).
13165 are used. The gross density of PU insulation boards with
multi­layer aluminium facings for building construction is 2.4 Delivery status
approx. 31 ­ 32 kg/m³.
Polyurethane insulation boards with multi­layer aluminium
The nominal thermal conductivity is 0.022 W/(m.K), the thermal
facings are manufactured with plane­parallel surfaces or as
conductivity design value which is used for calculating the
tapered insulation boards in a thickness range of 20 to 300 mm.
thermal performance of insulation layers in buildings is 0.023
This Product Declaration refers to a board thickness of 120
W/(m.K). In addition, the nominal value of the thermal mm. The format of the boards depends on the planned
resistance of RD = 5.45 (m².K)/W and the thickness of 22 mm application. The width can be up to 1250 mm and the length up
of the insulation board at RD = 1 (m².K)/W can be specified. to 12 m. This product declaration refers to a surface area of
1m2.
Nominal compressive stress or nominal compressive strength
at 10% deformation is 100 kPa (dh) or 150 kPa (ds) acc. to DIN 2.5 Base materials/Ancillary materials
4108-10. Higher compressive strength is possible. Nominal The 12 cm PU board with multi­layer aluminium facings
tensile strength perpendicular to the insulation board plane is consists of 3.71 kg/m² PU rigid foam and 0.33 kg/m² multi­layer
40 kPa. Higher tensile strength is possible. PU insulation aluminium facings. Polyurethane rigid foam is formed by the
boards with multi­layer aluminium facings are impermeable to chemical reaction of MDI (approx. 58 – 65 %) and polyol
water vapour and do not absorb moisture. Polyurethane rigid (approx. 26 – 31 %), adding low boiling point blowing agents
foam is a distinctive thermosetting material and therefore (approx. 3 – 6 %). Insulation boards with flexible facings are
cannot be melted. foamed exclusively with the hydrocarbon pentane. Due to the
closed­cell structure, the blowing agent remains within the foam
Constructional data
cells. Water (approx. 0.2 – 1.5 %), foam stabilisers and
catalysts (approx. 2 – 6 %), as well as flame retardants
(Phosphoric acid ester approx. 2 – 5 %) are added as ancillary
materials.
The raw materials used for the production of polyurethane rigid
foam are mainly obtained from crude oil, undergoing several
production stages. Alternatively, polyols and MDI can be
produced, in part, from renewable, plant­based raw materials or
recycled materials. This is not part of this product declaration.
Polyurethane rigid foam does not contain volatile isocyanates.
Under the current Regulation on the Registration, Evaluation,
Authorisation and Restriction of Chemicals (REACH)
polyurethane rigid foam is declared as follows:
2 Environmental Product Declaration ­ IVPU e.V. ­ PU thermal insulation boards with multi­layer aluminium facing
the PU wedges can be reused in the form of PU press plates.
• Polyurethane rigid foam contains substances listed in
the Candidate List
2.10 Condition of use
for authorization on 23 January 2024 exceeding 0.1
Under normal conditions of use, the material does not undergo
percentage by mass: no.
any changes in terms of substance during its service life time.
• Polyurethane rigid foam contains other carcinogenic,
Polyurethane is resistant to most chemicals used in
mutagenic, reprotoxic (CMR) substances in categories
construction and does not rot.
1A or 1B which are not on the candidate list, exceeding
0.1 percentage by mass: no 2.11 Environment and health during use
• Biocide products were added to this construction
The requirements of the Committee for Health­related
product or it has been treated with biocide products (this
Evaluation of Building Products (AgBB) are met. Measurements
then concerns a treated product as defined by the (EU)
of emissions using testing chambers in accordance with the
Ordinance on Biocide Products No. 528/2012): no
relevant testing norms (EN 16516) showed that volatile organic
substances (VVOC, VOC) are only emitted in small quantities.
Multi­layer aluminium facings consist of approx. equal shares of
aluminium, paper, and low density polyethylene (LDPE).
Regarding the current REACH candidate list, the foam
formulations contain no SVHC substances (see section 2.5).
2.6 Manufacture
Polyurethane rigid foam insulation boards with flexible multi­
Polyurethane insulation products are odourless.
layer aluminium facings are produced in a continuous process
on a double belt line. In this process, the polyurethane reaction 2.12 Reference service life
mixture pours from a mixing head onto the bottom facing where
When used properly, the service life time of polyurethane rigid
it foams up and glues – still within the line's pressure area –
foam corresponds to the service life time of the insulated
with the top multi­layer aluminium facing. After passing the
construction component or building. The performance of the
double belt line, the foam boards are cut to the desired
insulation boards stays constant throughout the entire service
dimensions.
life time.
Description of the influences on the ageing of the product when
Quality assurance
applied in accordance with the rules of technology.
The declared products are subject to quality controls. Quality
assurance is based on surveillance and certification by
independent Notified Bodies. 2.13 Extraordinary effects
Fire
2.7 Environment and health during manufacturing
According to national approvals, polyurethane insulation
No health protection measures extending beyond the legally­
products are classified either as class E or class C acc. to EN
mandated work protection measures for industrial businesses
13501-1. Pitched roof constructions with polyurethane
are required during the entire manufacturing process. No
insulation over rafters that comply with the classification report
special environmental protection measures apart from the legal
of IBS 316052507-A are classified as REI 30 (fire­retardant).
provisions are required.
Roof structures with top­side polyurethane insulation acc. to
DIN 18234-2 meet the fire­protection requirements stated in the
2.8 Product processing/Installation
Industrial Building Guideline even for fire containment or fire
Polyurethane insulation boards can be cut, sawed, milled, and
fighting sections with a roof surface of more than 2500 m².
abraded with conventional construction tools and portable
machines. In general, the boards are fixed mechanically
In case of fire, PU rigid foam does not tend to smoulder. When
(pitched and flat roofs, cavity core insulation). Alternatively, PU
exposed to heat, PU rigid foam carbonizes without dripping off
insulation boards can be laid loosely, e.g. on floors. Observing
burning droplets. When burning, sooty products, water vapour,
the manufacturer's recommendations, it is also possible to glue
carbon monoxide, carbon dioxide, nitrogen oxides, as well as
the boards together by using either hot­setting or cold­setting
hydrogen cyanide are formed as it is the case e. g. for sheep
adhesives. Joints between cut insulation boards on roof ridges,
wool.
hips or valleys are to be sealed with polyurethane in­situ foam
The toxicity of the combustion gases mainly depends on the
without thermal bridges.
amount of burned material in relation to the size of the room in
which the gases are distributed. It also depends on the
While sawing, abrading, and milling insulation boards, dust is
ventilation conditions in the affected area.
generated. If there is no sufficient ventilation, workers who carry
out these processes have to protect themselves by wearing an Fire Protection
appropriate dust filter mask (see leaflet of the Name Value
'Berufsgenossenschaft der Chemischen Industrie' on Building material class acc. to EN 13501­1 E ­ C
respiratory protection). Dust concentration in the air (general
Burning droplets acc. to EN 13501­1 d0, none
limit of dust concentration as per TRGS 900, Technische
Smoke gas development acc. to EN 13501­1 s1 ­ s3
Regeln für Gefahrstoffe) must not exceed the following values:
• 10 mg/m³ (measured as inhalable fraction)
• 1.25 mg/m³ (measured as alveolar fraction) Water
Due to the predominant closed­cell structure, insulation
These limits are time­weighted averages assuming an 8­hour products made of polyurethane rigid foam absorb water only in
exposure per day, 5 days a week, during working lifetime. small quantities. They are not hygroscopic, i.e. they do not
Cutting leftovers can be treated in a household waste absorb water vapour from the air. When unexpectedly exposed
incernation plant with energy recovery or they can be subject to to water (e.g. flood), only very small
a separate collection and a mechanical recycling process. amounts of soluble substances are emitted.
2.9 Packaging Mechanical destruction
Mainly, plastic foils and EPS or PU wedges are used as The disintegration of the poduct by mechanical processes does
packaging material. The plastic foils can be recycled whereas not have relevant effects on the environment.
3 Environmental Product Declaration ­ IVPU e.V. ­ PU thermal insulation boards with multi­layer aluminium facing
construction waste, are mechanically shredded and
2.14 Re-use phase subsequently pressed into board­shaped products while adding
Dismantling polyurethane insulation products as well as sorting binding agents. PU pressed adhesive boards are a high­quality
and waste identifying can be done without difficulties, since material that are used, among others, to insulate window
they are usually mounted mechanically or laid loosely. frames or thermal bridges.
Clean and undamaged polyurethane insulation boards can be 2.15 Disposal
reused as well as recycled mechanically or chemically According to the Waste Catalogue Ordinance, polyurethane
(glycolysis). Glycolysis means that polyurethane rigid foam insulatiin products shall not be disposed of without prior
waste is transformed into a fluid substance called glycolysis treatment. The waste code for construction waste is 170604.
polyol, which can be used again as raw material in the During thermal treatment, the energy content of the insulation
production of polyurethane. material can be recovered.
When reutilised from mechanical material recycling, 2.16 Further information
polyurethane rigid foam waste is used to produce press boards. Please visit www.ivpu.de and www.daemmt­besser.de for
In this process, cutting and mounting leftovers, as well as further information on PU insulation products.
3. LCA: Calculation rules
construction sites are handled using mainly material recycling
3.1 Declared Unit (see 2.15).
The declared unit is 1 m² of installed PU thermal insulation Using a worst­case approach, only the incineration and the
board with multi­layer aluminium facing (on both sides) and has consequent energy benefit beyond the system boundary have
the following specifications: been considered in this EPD.
Declared unit
3.4 Cut-off criteria
Name Value Unit
In this study, all available data from the production are taken
Declared unit 1 m2 into account, i.e. all used raw materials, used thermal energy,
Gross density of the PU foam 30.92 kg/m3 as well as electrical power consumption. Therefore, even
materials and power consumption levels that have a share of
Grammage 4.04 kg/m2
less than 1 % are considered.
Layer thickness 0.12 m
It can be assumed that all neglected processes put together
Design value of thermal conductivity 0.023 W/(mK) account for no more than 5 % of total power and mass
Thermal resistance (R­value) 5.45 m²•W/K consumption. The manufacturers have provided data on
transport expenditures for all relevant material flows. Machinery
Other declared units are allowed if the conversion is shown
and installations required for production are neglected.
transparently.
3.5 Background data
This EPD is based on weighted averages, which have been
Background data originates from the Sphera LCA FE (GaBi ts)
determined on the basis of the single values originating from
software database CUP 2023.2 from Sphera. The power mix
the factories of the IVPU members. Average energy
with different countries has been used. The last revision of the
consumption for producing PU boards has been weighted
used data was less than 6 years ago.
according to the quantities of produced PU rigid foam in m3.
Raw material consumption has been weighted according to 3.6 Data quality
used quantities in kg. Rigid foam waste is weighted according The data used are primary data originating from the industry
to the quantities of produced PU rigid foam in m3 whereas and were gathered by the IVPU in 2018. 8 IVPU members
facing waste is weighted according to used quantities of facings participated in this data gathering. 2 additional IVPU members
in m2. joined the study in this update with data gathered in 2023. The
IVPU represents more than 90 % of the companies within the
3.2 System boundary German polyurethane insulation products market. This EPD is
The type of EPD according to EN15804 is cradle to gate with based on weighted averages, which have been determined on
options, modules C1­C4, and module D. the basis of the single values originating from the factories of
Life cycle assessment considers the following steps of the life the aforementioned manufacturing companies.
cycle: The data's quality as well as its temporal, technological and
• Production and supply of raw materials (A1) geographical representativeness can be classified as good.
• Transporting raw materials (A2)
3.7 Period under review
• Production including packaging (A3)
The data basis is based on production data from 2018 and
• Transport to construction site (A4)
2023.
• Installation in buildings (thermal treatment of packaging
The used quantities of raw materials, energy, as well as
waste) (A5)
ancillary materials and fuels are averages compiled over a time
• Transport to End­of­Life (C2)
span of 12 months.
• Waste treatment: energy for shredders (C3)
• Thermal treatment (PU foam) (C3)
3.8 Geographic Representativeness
• Recycling or use potentials beyond the system's
Land or region, in which the declared product system is
boundary (D).
manufactured, used or handled at the end of the product´s
3.3 Estimates and assumptions lifespan: Germany
For all inputs, specific Sphera LCA FE (GaBi ts) datasets were
available. 3.9 Allocation
Currently, waste from PU foam production generated in
4 Environmental Product Declaration ­ IVPU e.V. ­ PU thermal insulation boards with multi­layer aluminium facing
When thermally treated in waste incineration plants (MVA),
recycling as well as use potentials beyond the system boundary 3.10 Comparability
for power and thermal energy in module D are taken into Basically, a comparison or an evaluation of EPD data is only
account in an input­specific manner considering elemental possible if all the data sets to be compared were created
composition as well as thermal values. Due to manufacturing according to EN 15804 and the building context, respectively
locations and distribution throughout all of Europe, the the product­specific characteristics of performance, are taken
substitution processes refer to reference area EU­27. into account. The used background database is Sphera LCA
FE (GaBi ts), CUP 2023.2.
4. LCA: Scenarios and additional technical information
Installation in buildings (A5)
Characteristic product properties of biogenic carbon
The biogenic carbon content declared is provided below. No Name Value Unit
biogenic carbon content exists in the product, only packaging Packaging waste 0.53 kg
materials.
Information on describing the biogenic carbon content at
End of life cycle (C1-C4)
factory gate
Name Value Unit
Name Value Unit
Waste processing (C3) energy for shredders 0.808 MJ
kg
Biogenic carbon content in product ­ Reuse ­ kg
C
Recycling (aluminium content of facing) 0.33 kg
Biogenic carbon content in accompanying kg
packaging 0.0185 C Energy recovery 3.71 kg
Landfilling ­ kg
Note: 1 kg of biogenic carbon is equivalent to 44/12 kg of CO2.
Module C1 considers a manual demolition (without any
burden). Upon removal from the building, products are
The following technical scenario information is used to calculate assumed to be transported 100 km (module C2) to a recycling
the declared modules. The values refer to the declared unit of facility. The foam waste in the EoL phase is sent to a waste
1m² of installed PU thermal insulation board with multi­layer incineration plant.
aluminium facing.
The waste is shredded and incinerated. These processes are
Transport to construction site (A4)
grouped to module C3. Resulting potential benefits for
Name Value Unit
electricity and thermal energy due to the incineration are
Litres of fuel 0.0262 l/100km grouped to module D.
Transport distance 500 km
Gross density of products transported 30.92 kg/m3 Aluminum facings are recycled. The recycling including the
recycling effort and the potential benefits are addressed in
Capacity utilisation (including empty runs) 85 %
module D.
5 Environmental Product Declaration ­ IVPU e.V. ­ PU thermal insulation boards with multi­layer aluminium facing
5. LCA: Results
DESCRIPTION OF THE SYSTEM BOUNDARY (X = INCLUDED IN LCA; MND = MODULE OR INDICATOR NOT DECLARED; MNR
= MODULE NOT RELEVANT)
Benefits and
Construction loads beyond
Product stage Use stage End of life stage
process stage the system
boundaries
la ire ta m w a Ry lp p u s tro p s n a rT g n iru tc a fu n a M e h t m o rf tro p s n a rTe tis e h t o t e ta g y lb m e s s A e s U e c n a n e tn ia M ria p e R tn e m e c a lp e R tn e m h s ib ru fe R y g re n e la n o ita re p Oe s u re ta w la n o ita re p Oe s u n o itc u rts n o c ­e Dn o itilo m e d tro p s n a rT g n is s e c o rp e ts a W la s o p s iD ­e s u e R­y re v o c e R­g n ilc y c e Rla itn e to p
A1 A2 A3 A4 A5 B1 B2 B3 B4 B5 B6 B7 C1 C2 C3 C4 D
X X X X X MND MND MNR MNR MNR MND MND X X X X X
RESULTS OF THE LCA - ENVIRONMENTAL IMPACT according to EN 15804+A2: 1 m² of installed PU board with multi-layer
aluminium facing
Parameter Unit A1-A3 A4 A5 C1 C2 C3 C4 D
GWP­total kg CO 2 eq 1.16E+01 4.43E­01 1.84E­01 0 8.73E­02 8.8E+00 0 ­3.75E+00
GWP­fossil kg CO 2 eq 1.19E+01 4.38E­01 1.82E­01 0 8.63E­02 8.51E+00 0 ­3.73E+00
GWP­biogenic kg CO 2 eq ­3.57E­01 1.02E­03 1.74E­03 0 2.02E­04 2.9E­01 0 ­1.47E­02
GWP­luluc kg CO 2 eq 1.03E­02 4.14E­03 1.88E­07 0 8.16E­04 2.3E­05 0 ­2.8E­04
ODP kg CFC11 eq 2.4E­11 3.92E­14 8.86E­15 0 7.71E­15 2.08E­12 0 ­2.6E­11
AP mol H+ eq 2.42E­02 5.84E­04 2.1E­05 0 1.15E­04 5.11E­03 0 ­5.83E­03
EP­freshwater kg P eq 5.27E­05 1.63E­06 2.13E­09 0 3.21E­07 4.71E­07 0 ­5.47E­06
EP­marine kg N eq 6.53E­03 2.05E­04 5.57E­06 0 4.05E­05 2.42E­03 0 ­1.52E­03
EP­terrestrial mol N eq 6.67E­02 2.47E­03 1.02E­04 0 4.86E­04 2.8E­02 0 ­1.63E­02
kg NMVOC
POCP 3.47E­02 5.04E­04 1.57E­05 0 9.92E­05 6.22E­03 0 ­4.28E­03
eq
ADPE kg Sb eq 1.33E­06 2.91E­08 8.25E­11 0 5.72E­09 1.81E­08 0 ­2.53E­07
ADPF MJ 3.1E+02 6.08E+00 2.27E­02 0 1.2E+00 3.82E+00 0 ­6.65E+01
m3 world eq
WDP 1.83E+00 5.16E­03 1.65E­02 0 1.02E­03 8.76E­01 0 ­3.36E­01
deprived
GWP = Global warming potential; ODP = Depletion potential of the stratospheric ozone layer; AP = Acidification potential of land and water; EP =
Eutrophication potential; POCP = Formation potential of tropospheric ozone photochemical oxidants; ADPE = Abiotic depletion potential for non­fossil
resources; ADPF = Abiotic depletion potential for fossil resources; WDP = Water (user) deprivation potential)
RESULTS OF THE LCA - INDICATORS TO DESCRIBE RESOURCE USE according to EN 15804+A2: 1 m² of installed PU board
with multi-layer aluminium facing
Parameter Unit A1-A3 A4 A5 C1 C2 C3 C4 D
PERE MJ 2.59E+01 4.31E­01 6.72E­01 0 8.48E­02 1.36E+00 0 ­1.96E+01
PERM MJ 6.67E­01 0 ­6.67E­01 0 0 0 0 0
PERT MJ 2.66E+01 4.31E­01 5.66E­03 0 8.48E­02 1.36E+00 0 ­1.96E+01
PENRE MJ 1.9E+02 6.1E+00 2.1E+01 0 1.2E+00 1.03E+02 0 ­6.65E+01
PENRM MJ 1.21E+02 0 ­2.1E+01 0 0 ­9.96E+01 0 0
PENRT MJ 3.11E+02 6.1E+00 2.27E­02 0 1.2E+00 3.82E+00 0 ­6.65E+01
SM kg 0 0 0 0 0 0 0 0
RSF MJ 0 0 0 0 0 0 0 0
NRSF MJ 0 0 0 0 0 0 0 0
FW m3 8.41E­02 4.75E­04 3.87E­04 0 9.34E­05 2.1E­02 0 ­1.85E­02
PERE = Use of renewable primary energy excluding renewable primary energy resources used as raw materials; PERM = Use of renewable primary
energy resources used as raw materials; PERT = Total use of renewable primary energy resources; PENRE = Use of non­renewable primary energy
excluding non­renewable primary energy resources used as raw materials; PENRM = Use of non­renewable primary energy resources used as raw
materials; PENRT = Total use of non­renewable primary energy resources; SM = Use of secondary material; RSF = Use of renewable secondary fuels;
NRSF = Use of non­renewable secondary fuels; FW = Use of net fresh water
RESULTS OF THE LCA – WASTE CATEGORIES AND OUTPUT FLOWS according to EN 15804+A2:
1 m² of installed PU board with multi-layer aluminium facing
Parameter Unit A1-A3 A4 A5 C1 C2 C3 C4 D
HWD kg 1.41E­07 2.26E­11 6.29E­13 0 4.44E­12 7.41E­11 0 ­3.57E­09
NHWD kg 3.8E­01 8.79E­04 7.59E­04 0 1.73E­04 4.89E­02 0 ­1.43E­01
RWD kg 4.78E­03 7.89E­06 1.33E­06 0 1.55E­06 3.35E­04 0 ­5.11E­03
CRU kg 0 0 0 0 0 0 0 0
MFR kg 0 0 0 0 0 6.09E­02 0 0
MER kg 0 0 0 0 0 0 0 0
EEE MJ 0 0 3.73E­01 0 0 1.49E+01 0 0
6 Environmental Product Declaration ­ IVPU e.V. ­ PU thermal insulation boards with multi­layer aluminium facing
EET MJ 0 0 6.63E­01 0 0 2.7E+01 0 0
HWD = Hazardous waste disposed; NHWD = Non­hazardous waste disposed; RWD = Radioactive waste disposed; CRU = Components for re­use;
MFR = Materials for recycling; MER = Materials for energy recovery; EEE = Exported electrical energy; EET = Exported thermal energy
RESULTS OF THE LCA – additional impact categories according to EN 15804+A2-optional:
1 m² of installed PU board with multi-layer aluminium facing
Parameter Unit A1-A3 A4 A5 C1 C2 C3 C4 D
Disease
PM 2.17E­07 4.85E­09 1.11E­10 0 9.54E­10 1.54E­08 0 ­5.29E­08
incidence
IR kBq U235 eq 5.04E­01 1.14E­03 2.14E­04 0 2.24E­04 5.48E­02 0 ­8.77E­01
ETP­fw CTUe 1.05E+02 4.29E+00 8.73E­03 0 8.44E­01 1.1E+00 0 ­1.01E+01
HTP­c CTUh 3.39E­09 8.64E­11 1.16E­12 0 1.7E­11 8.24E­11 0 ­8.64E­10
HTP­nc CTUh 1.32E­07 3.81E­09 9.5E­12 0 7.51E­10 1.26E­09 0 ­2.06E­08
SQP SQP 8.5E+01 2.54E+00 6.97E­03 0 5E­01 1.11E+00 0 ­1.18E+01
PM = Potential incidence of disease due to PM emissions; IR = Potential Human exposure efficiency relative to U235; ETP­fw = Potential comparative
Toxic Unit for ecosystems; HTP­c = Potential comparative Toxic Unit for humans (cancerogenic); HTP­nc = Potential comparative Toxic Unit for humans
(not cancerogenic); SQP = Potential soil quality index
Disclaimer 1 – for the indicator “Potential Human exposure efficiency relative to U235”. This impact category deals mainly with the
eventual impact of low­dose ionizing radiation on human health of the nuclear fuel cycle. It does not consider effects due to possible
nuclear accidents, occupational exposure or radioactive waste disposal in underground facilities. Potential ionizing radiation from the
soil, radon and from some construction materials is also not measured by this indicator.
Disclaimer 2 – for the indicators “abiotic depletion potential for non­fossil resources”, “abiotic depletion potential for fossil resources”,
“water (user) deprivation potential, deprivation­weighted water consumption”, “potential comparative toxic unit for ecosystems”,
“potential comparative toxic unit for humans – cancerogenic”, “Potential comparative toxic unit for humans ­ not cancerogenic”,
“potential soil quality index”. The results of this environmental impact indicator shall be used with care as the uncertainties on these
results are high as there is limited experience with the indicator.
6. LCA: Interpretation
Modules A1­A3: The environmental impacts during the MVAs which burn PU cores inorder to generate power and
production stage are mainly determined by raw material steam. Additionally, Module D possesses the recycling potential
production and processing in Module A1. For nearly all of the aluminium used.
categories, these impacts can mostly be attributed to the PU
foam (approx. 80 %) and to a lesser extent to the multi­layer The LCA results show high robustness since the primary data,
aluminium facings (< 10 %). More specifically, the results are they are based on, do not show any outliers in terms of energy
mainly driven the production of MDI and polyols in almost all consumption and product's composition while comparing the
indicators except for ODP and POCP, where the impacts can contributing companies and sites. All background data are
mainly be attributed to the power mix and the other production sourced from Sphera LCA FE (GaBi ts) databases. With the
expenses, respectively. used data sets a good overall representativity with regards to
completeness, geographical coverage and technological
Module D: The utilization potential for the next product coverage is ensured.
systemoriginates from using primary energy generated from
7. Requisite evidence
7.2 Isocyanate emission
7.1 VOC emissions In the analysis conducted by the Fraunhofer Institut für
Emission tests on PU boards with multi­layer aluminium facings Holzforschung, Wilhelm­Klauditz­Institut WKI (Test report No.
found that the VOC values are significantly below the limits 861-98), no isocyanate emission could be detected in the 1m³
determined by the AgBB scheme (PU Europe Technical test chamber. SUPELCO cartridges have been used for
Dossier). The tests were conducted by the research detecting MDI. The detection limit is at 10 ng/m³.
organisations Eurofins (Denmark), VTT (Finland) and
Fraunhofer WKI (Germany), Test report No. MAIC­2016­3308, 7.3 Formaldehyde
among others. Emission tests on PU insulation boards only detected very
small quantities of formaldehydes (< 3 μg/m³ (PU Europe
VOC emissions
Technical Dossier)). This is significantly below the threshold
Name Value Unit
value of 120 μg/m³ (Class E1).
TVOC (C6 ­ C16) 0 ­ 100 μg/m3
Sum SVOC (C16 ­ C22) 0 ­ 10 μg/m3
R (dimensionless) 0 ­ 0.5 ­
VOC without NIK 0 ­ 100 μg/m3
Carcinogenic Substances ­ μg/m3
8. References
Standards DIN 4108­4:2020­11, Thermal insulation and energy economy
in buildings ­ Part 4: Hygrothermal design values.
DIN 4108-4
7 Environmental Product Declaration ­ IVPU e.V. ­ PU thermal insulation boards with multi­layer aluminium facing
DIN 4108-10
DIN 4108­10:2021­11, Thermal insulation and energy economy prEN 16783:2022-12 - draft
in buildings ­ Part 10: Application­related requirements for Thermal insulation products ­ Environmental Product
thermal insulation materials ­ Factory­made products. Declarations (EPD) ­ Product Category Rules (PCR)
complementary to EN 15804 for factory made and in­situ
EN 12091 formed products
EN 12091:2013­06, Thermal insulating products for building
applications ­ Determination of freeze­thaw resistance. EN ISO 14025
EN ISO 14025:2011, Environmental labels and declarations —
EN 13165 Type III environmental declarations —
EN 13165:2016­09, Thermal insulation products for buildings – Principlesandprocedures.
Factory­made rigid polyurethane foam (PU) products ­
Specification; German version EN 13165:2012. (This norm Further References
covers polyurethane rigid foam (PUR) and polyisocyanurate
rigid foam (PIR)). AgBB
Evaluation scheme for VOCs from construction products;
DIN EN 13501-1 approach for assessing health risks caused by volatile organic
EN 13501­1:2019­05, Fire classification of construction compounds (VOCs and SVOCs) from construction products,
products and building elements ­ Part 1: Classification using version 2021.
data from reaction to fire tests; German version EN 13501­
1:2007+A1:2010. Waste Catalogue Ordinance
Waste Catalogue Ordinance of 10 Dec 2001 (Federal Law
EN 14308 Gazette I p. 3379), last amended by Article 2 of the Ordinance
EN 14308:2016­03, Thermal insulation products for building of 24 July 2002 (Federal Law Gazette 2833)
equipment and industrial installations ­ Factory made rigid
polyurethane foam (PUR) and polyisocyanurate foam (PIR) CPR
products. Regulation (EU) No. 305/2011 of the European Parliament and
of the Council of 9 March 2011 laying down hamonised
EN 15801 condition for the marketing of construction products and
EN 15801:2010­04, Conservation of cultural property ­ Test repealing Council Directive 89/106/EC.
methods ­ Determination of water absorption by capillarity.
EXCLI Journal
EN 1606 Hoffmann, Hans­Dieter; Schupp, Thomas: 'Evaluation of
EN 1606:2013­05, Thermal insulating products for building consumer risk resulting from exposure against MDI from
applications ­ Determination of compressive creep. polyurethane foam,' scientific article, published in the EXCLI
Journal in 2009.
EN 1607
EN 1607:2013­05, Thermal insulating products for building IBU 2021
applications ­ Determination of tensile strength perpendicular to Institut Bauen und Umwelt e.V.: General Instructions for the
faces. EPD programme of Institut Bauen und Umwelt e.V., version 2.0,
Berlin: Institut Bauen und Umwelt e.V., 2021
EN 16516 www.ibu­­epd.com
EN 16516:2020­10, Construction products: Assessment of
release of dangerous substances ­ Determination of emissions IBS 316052507-A
into indoor air. IBS Linz: Test report No. 316052507­A, dated 06.04.2017
(IVPU), "Report on the classification of fire resistance of a rafter
DIN 18234-2 roof with PU over­rafter insulation".
DIN 18234­2:2018­05, Fire safety of large roofs for buildings ­
Fire exposure from below ­ Part 2: List of roofs which fulfil the IVPU news
requirements of DIN 18234­1; roof areas without openings. Article "Report on emission of volatile components from PUR
rigid foam insulation products" no. 64 dated June 1999.
EN 29052-1
EN 29052­1:1992­08, Acoustics; determination of dynamic PCR Part A
stiffness; part 1: materials used under floating floors in PCR ­ Part A: Calculation rules for the Life Cycle Assessment
dwellings. and Requirements on the Background Report, version 1.3,
Institut Bauen und Umwelt e.V., 2021.
EN 826
EN 826:2013­05, Thermal insulating products for building PCR Part B
applications ­ Determination of compression behaviour. PCR ­ Part B: Requirements of the EPD for foam
plasticsinsulation materials, v8, 2021 www.bau­­umwelt.de
EN 12088
EN 12088:2013, Thermal insulating products for building PU Europe Technical Dossier
applications ­ Determination of long term water absorption by Technical Dossier for amendment to mandate M103
diffusion. VOC/SVOC emissions, doc. 13/241, 2013.
EN 15804 Ordinance on Biocide Products No. 528/2012
EN 15804:2012+A2:2019+AC:2021, Sustainability of Regulation (EU) No. 528/2012 of the European Parliament and
construction works — Environmental Product Declarations Core of the Council of 22 May 2012 concerning the making available
rules for the product category of construction products. on the market and use of biocidal products.
8 Environmental Product Declaration ­ IVPU e.V. ­ PU thermal insulation boards with multi­layer aluminium facing
REACH Commission proposal for the classification of emissions from
Regulation (EC) No. 1907/2006 of the European Parliament building products in the European Union".
and of the Council dated 18th December 2006 on the
Registration, Evaluation, Test report No. 861-98
Authorisation and Restriction of Chemicals (REACH). Fraunhofer Institut für Holzforschung, Wilhelm­Klauditz­Institut
(WKI): Test report No. 861­98, dated 07.12.1998 (IVPU), "Test
Sphera LCA FE (GaBi ts) reports on emissions of volatile components from polyurethan
Sphera LCA for Experts, LCA FE, software­ system and insulating materials".
databases, Managed LCA content MLC (fka GaBi database),
University of Stuttgart and Sphera Solutions GmbH, 2023 TRGS 900
CUPVersion: 2023.2, MLC data set documentation Federal Institute for Occupational Safety and Health: Technical
underhttps://sphera.com/product­sustainability­gabi­data Rules for Hazardous Substances (TRGS) 900, Threshold
search/ (March 2024). values for workplaces, 2006, last modified 15.01.204
The literature referred to in the Environmental Product
Test report No. MAIC-2016-3308 Declaration must be listed in full.Standards already fully quoted
Fraunhofer Institut für Holzforschung, Wilhelm­Klauditz­Institut in the EPD do not need to be listed here again.
(WKI): Test report No. MAIC­2016­3308, dated 04.08.2016 (PU The current version of PCR Part A and PCR Part B of the PCR
Europe), "Evaluation of emissions data from PU insulation on a document on which they are based must be referenced.
9 Environmental Product Declaration ­ IVPU e.V. ­ PU thermal insulation boards with multi­layer aluminium facing
Publisher
Institut Bauen und Umwelt e.V. +49 (0)30 3087748­ 0
Hegelplatz 1 info@ibu­epd.com
10117 Berlin www.ibu­epd.com
Germany
Programme holder
Institut Bauen und Umwelt e.V. +49 (0)30 3087748­ 0
Hegelplatz 1 info@ibu­epd.com
10117 Berlin www.ibu­epd.com
Germany
Author of the Life Cycle Assessment
Sphera Solutions GmbH +49 711 341817­0
Hauptstraße 111­ 113 info@sphera.com
70771 Leinfelden­Echterdingen www.sphera.com
Germany
Owner of the Declaration
IVPU ­ Industrieverband Polyurethan­Hartschaum +49 711 29 17 16
e.V. ivpu@ivpu.de
Heilbronner Str. 154 http://www.ivpu.de/
70191 Stuttgart
Germany
10 Environmental Product Declaration ­ IVPU e.V. ­ PU thermal insulation boards with multi­layer aluminium facing
