ENVIRONMENTAL PRODUCT DECLARATION
as per ISO 14025 and EN 15804+A2
Owner of the Declaration KONE Corporation
Publisher Institut Bauen und Umwelt e.V. (IBU)
Programme holder Institut Bauen und Umwelt e.V. (IBU)
Declaration number EPD-KON-20230580-CBA2-EN
Issue date 22.12.2023
Valid to 14.03.2028
Sliding Door 50 / 50E / 50T / 50ET / 50L / 50 LT
KONE
www.ibu-epd.com | https://epd-online.com
General Information
KONE Sliding Door 50 / 50E / 50T / 50ET / 50L / 50 LT
Programme holder Owner of the declaration
IBU – Institut Bauen und Umwelt e.V. KONE Corporation
Hegelplatz 1 Keilasatama 3
10117 Berlin 02150 ESPOO
Germany Finland
Declaration number Declared product / declared unit
EPD-KON-20230580-CBA2-EN The declared unit is one piece of the sliding door system 50 without drive
comprising:
• Sliding panels
• Side screens
• Product packaging
This declaration is based on the product category rules: Scope:
Automatic doors, automatic gates, and revolving door systems, This EPD refers to the entire life cycle of a specific sliding door system 50.
01.08.2021 The EPD is also representative for the sliding doors 50E / 50T / 50ET / 50L
(PCR checked and approved by the SVR) and 50LT. The production location is in Germany. Green electricity is used
a the production facility.
Issue date The year of data collection is 2022.
22.12.2023
The owner of the declaration shall be liable for the underlying information
and evidence; the IBU shall not be liable with respect to manufacturer
information, life cycle assessment data and evidences.
Valid to
14.03.2028 The EPD was created according to the specifications of EN 15804+A2. In
the following, the standard will be simplified as EN 15804.
Verification
The standard EN 15804 serves as the core PCR
Independent verification of the declaration and data according to ISO
14025:2011
internally X externally
Dipl.-Ing. Hans Peters
(Chairman of Institut Bauen und Umwelt e.V.)
Florian Pronold Dr.-Ing. Wolfram Trinius,
(Managing Director Institut Bauen und Umwelt e.V.) (Independent verifier)
1 Environmental Product Declaration - KONE - Sliding Door 50 / 50E / 50T / 50ET / 50L / 50 LT
Product
Product description/Product definition Performance data of the product with respect to its
The automatic sliding doors have a slim, thermal divided profile characteristics in accordance with the relevant technical
system. Therefore, heat insulation is achieved without provision which can be applied are mentioned above.
compromising in the slim profile. The sliding doors make The Sliding Door 50 comprises the following components
considerable savings of the running energy and heating costs including packaging:
possible, as well as a reduction in CO2- emissions for the entire
use phase. Base materials/Ancillary materials
Name Value Unit
To meet all requirements, the systems can be combined with
Glass 81 %
different operator versions. For the sliding door series 50 the
Aluminium 12 %
standards which can be applied are the following:
Steel 1 %
• EN 16005
Plastics 6 %
• DIN 18650-1/ -2
• ISO 13849-1 The sliding doors contain partial articles which contain
• EN 60335-1 substances listed in the Candidate List of REACH Regulation
• EN 60335-2-103 1907/2006/EC (date: 17.01.2023) exceeding 0.1 percentage by
• IEC 60335-2-103 mass: no
• 2011/65/EU (RoHS)
The Candidate List can be found on the ECHA website
Application address: https://echa.europa.eu/de/home.
The sliding door system is used in particular where energy
saving enjoys key significance during the reference service life.
Each system is manufactured to the individual dimensions of
the respective building project.
Technical Data
Following data are applicable for the sliding panels and side Reference service life
screens: The reference service life amounts to 10 years, depending on
• Heat transition coeffizient (U-value) for the sliding door the application and frequency of use. Regular maintenance is
system measuring 6250 x 3305: 1,4 [W/m²K] advised to ensure the life expactancy of 10 years. For repairs
• Heat transition coeffizient (U-value) for the sliding door and renewals, suitable spare parts are available. The sliding
system measuring 2100 x 2205: 1,6 [W/m²K] door system 50 is tested and certified according to EN 16005,
• Insulation glass units: 1,0 [W/m²K] meaning they are desingned to withstand a minimum of
1.000.000 cycles.
LCA: Calculation rules
construction process stage.
Declared Unit
The declared unit is 1 piece of the product: Sliding Door 50 Use stage - Module B6
Name Value Unit The use stage related to the operation of the building includes:
Declared unit 1 pce. — B6, operational energy use
Mass (total system) 287.43 kg
End-of-life stage– Modules C1-C4 and D
The end-of-life stage includes:
System boundary
— C1, de-construction, demolition:
The type of EPD is: cradle-to-gate with options, modules C1–
— C2, transport to waste processing;
C4, and module D (A1–A3 + C + D and additional modules: A4
— C3, waste processing for reuse, recovery and/or recycling;
+ A5 + B6)
— C4, disposal; including provision and all transport, provision
of all materials, products and related energy and water use.
Production - Module A1-A3
Module D (Benefits and loads beyond the system boundary)
The product stage includes:
includes:
— A1, raw material extraction, processing and mechanical
— D, recycling potentials, expressed as net impacts and
treatments, processing of secondary material input (e.g.
benefits.
recycling processes),
— A2, transport to the manufacturer, Geographic Representativeness
— A3, manufacturing and assembly including provision of all Land or region, in which the declared product system is
materials, products and energy, as well as waste processing up manufactured, used or handled at the end of the product´s
to the end-of waste state. lifespan: Global
Construction stage - Modules A4-A5
The construction process stage includes: Comparability
— A4, transport to the building site; Basically, a comparison or an evaluation of EPD data is only
— A5, installation into the building; including provision of all possible if all the data sets to be compared were created
materials, products and energy, as well as waste processing up according to EN 15804 and the building context, respectively
to the end-of waste state or disposal of final residues during the the product-specific characteristics of performance, are taken
2 Environmental Product Declaration - KONE - Sliding Door 50 / 50E / 50T / 50ET / 50L / 50 LT
into account. Background database: GaBi, SP40.
LCA: Scenarios and additional technical information
not declared. The results for the drive unit are shown in a
Characteristic product properties of biogenic carbon separate EPD.
Information on describing the biogenic Carbon Content at
factury gate End of life (C1-C4)
Name ValueUnit C1: The product expansion depends on the building. The
Biogenic carbon content in accompanying kg product share is so low that noenvironmental burden is
0.003
packaging C assumed.
Name Value Unit
Note: 1 kg of biogenic carbon is equivalent to 44/12 kg of CO .
2
Collected separately waste type waste type 278 kg
Recycling 36.4 kg
The following technical scenario information is required for the Energy recovery 7.59 kg
declared modules. Landfilling 234 kg
Transport to the building site (A4) Transport to waste management 50 km
Name Value Unit The product is disassembled in a recycling process. Material
Litres of fuel (per 1 kg) 0.00276 l/100km recycling is then assumed for the metals, electronics and
Transport distance via medium truck 100 km electromechanics. The plastic components are assumed to be
incinerated with energy recovery. Glass and minor proportions
Capacity utilisation (including empty runs) 55 %
of residues arising from the recycling process are landfilled.
Transport distance is declared for a distance of 100km by truck Region for the End of Life is: Global.
in order to allow scaling to a specific point of installation.
Reuse, recovery and/or recycling potentials (D), relevant
Installation into the building (A5) scenario information
Name Value Unit The collection rate is 100%.
Waste packaging (paper and plastic) 9 kg Name Value Unit
Reference service life
Name Value Unit
Life Span according to the manufacturer 10 a
Operational energy use (B6)
The drive unit is not included in this EPD, which is why B6 is
3 Environmental Product Declaration - KONE - Sliding Door 50 / 50E / 50T / 50ET / 50L / 50 LT
LCA: Results
DESCRIPTION OF THE SYSTEM BOUNDARY (X = INCLUDED IN LCA; MND = MODULE OR INDICATOR NOT DECLARED; MNR
= MODULE NOT RELEVANT)
Benefits and
Construction loads beyond
Product stage Use stage End of life stage
process stage the system
boundaries
la ire ta m w a Ry lp p u s tro p s n a rT g n iru tc a fu n a M e h t m o rf tro p s n a rTe tis e h t o t e ta g y lb m e s s A e s U e c n a n e tn ia M ria p e R tn e m e c a lp e R tn e m h s ib ru fe R y g re n e la n o ita re p Oe s u re ta w la n o ita re p Oe s u n o itc u rts n o c -e Dn o itilo m e d tro p s n a rT g n is s e c o rp e ts a W la s o p s iD -e s u e R-y re v o c e R-g n ilc y c e Rla itn e to p
A1 A2 A3 A4 A5 B1 B2 B3 B4 B5 B6 B7 C1 C2 C3 C4 D
X X X X X MND MND MNR MNR MNR MND MND X X X X X
RESULTS OF THE LCA - ENVIRONMENTAL IMPACT according to EN 15804+A2: 1 piece Sliding Door 50 / 50E / 50T / 50ET /
50L / 50 LT
Parameter Unit A1-A3 A4 A5 C1 C2 C3 C4 D
GWP-total kg CO 2 eq 5.1E+02 2.51E+00 2.29E+01 0 1.22E+00 1.93E+01 3.58E+00 -6.37E+01
GWP-fossil kg CO 2 eq 5.07E+02 2.4E+00 2.29E+01 0 1.16E+00 1.93E+01 3.56E+00 -6.35E+01
GWP-biogenic kg CO 2 eq 2.25E+00 1.11E-01 5.33E-04 0 5.4E-02 4.5E-04 1.2E-02 -1.79E-01
GWP-luluc kg CO 2 eq 1.97E-01 5.72E-05 1E-03 0 2.77E-05 1E-03 1E-02 -2E-02
ODP kg CFC11 eq 3.11E-09 2.54E-16 1.15E-14 0 1.23E-16 9.73E-15 1.32E-14 -3.36E-10
AP mol H+ eq 3.35E+00 2E-03 4E-03 0 1E-03 3E-03 2.6E-02 -1.89E-01
EP-freshwater kg P eq 4.72E-04 5.14E-07 1.84E-06 0 2.49E-07 1.55E-06 6.11E-06 -4.49E-05
EP-marine kg N eq 7.46E-01 7.65E-04 9.18E-04 0 3.71E-04 7.75E-04 7E-03 -2.8E-02
EP-terrestrial mol N eq 8.5E+00 9E-03 1.9E-02 0 4E-03 1.6E-02 7.2E-02 -3.08E-01
kg NMVOC
POCP 1.62E+00 2E-03 3E-03 0 1E-03 2E-03 2E-02 -8.8E-02
eq
ADPE kg Sb eq 2.46E-04 7.21E-08 1.58E-07 0 3.49E-08 1.34E-07 3.19E-07 -6.18E-05
ADPF MJ 7.32E+03 3.41E+01 1.06E+01 0 1.65E+01 8.95E+00 4.67E+01 -9.55E+02
m3 world eq
WDP 3.07E+01 5E-03 2.34E+00 0 2E-03 1.97E+00 3.73E-01 -3.98E+00
deprived
GWP = Global warming potential; ODP = Depletion potential of the stratospheric ozone layer; AP = Acidification potential of land and water; EP =
Eutrophication potential; POCP = Formation potential of tropospheric ozone photochemical oxidants; ADPE = Abiotic depletion potential for non-fossil
resources; ADPF = Abiotic depletion potential for fossil resources; WDP = Water (user) deprivation potential)
RESULTS OF THE LCA - INDICATORS TO DESCRIBE RESOURCE USE according to EN 15804+A2: 1 piece Sliding Door 50 /
50E / 50T / 50ET / 50L / 50 LT
Parameter Unit A1-A3 A4 A5 C1 C2 C3 C4 D
PERE MJ 7.88E+02 1.07E-01 2.76E+00 0 5.2E-02 2.33E+00 6.11E+00 -3.52E+02
PERM MJ 0 0 0 0 0 0 0 0
PERT MJ 7.88E+02 1.07E-01 2.76E+00 0 5.2E-02 2.33E+00 6.11E+00 -3.52E+02
PENRE MJ 6.77E+03 3.41E+01 3.98E+02 0 1.65E+01 1.73E+02 4.67E+01 -9.56E+02
PENRM MJ 5.51E+02 0 -3.87E+02 0 0 -1.64E+02 0 0
PENRT MJ 7.32E+03 3.41E+01 1.06E+01 0 1.65E+01 8.95E+00 4.67E+01 -9.56E+02
SM kg 2.86E+01 0 0 0 0 0 0 0
RSF MJ 0 0 0 0 0 0 0 0
NRSF MJ 0 0 0 0 0 0 0 0
FW m3 1.75E+00 1.93E-04 5.6E-02 0 9.34E-05 4.7E-02 1.2E-02 -5.83E-01
PERE = Use of renewable primary energy excluding renewable primary energy resources used as raw materials; PERM = Use of renewable primary
energy resources used as raw materials; PERT = Total use of renewable primary energy resources; PENRE = Use of non-renewable primary energy
excluding non-renewable primary energy resources used as raw materials; PENRM = Use of non-renewable primary energy resources used as raw
materials; PENRT = Total use of non-renewable primary energy resources; SM = Use of secondary material; RSF = Use of renewable secondary fuels;
NRSF = Use of non-renewable secondary fuels; FW = Use of net fresh water
RESULTS OF THE LCA – WASTE CATEGORIES AND OUTPUT FLOWS according to EN 15804+A2:
1 piece Sliding Door 50 / 50E / 50T / 50ET / 50L / 50 LT
Parameter Unit A1-A3 A4 A5 C1 C2 C3 C4 D
HWD kg 1.26E-05 3.31E-09 4.04E-08 0 1.6E-09 3.41E-08 7.11E-07 -2.51E-06
NHWD kg 6.46E+01 3E-03 2.38E+00 0 2E-03 2E+00 2.35E+02 -1.12E+01
RWD kg 1.6E-01 3.66E-05 3.94E-04 0 1.77E-05 3.32E-04 5.31E-04 -9E-02
CRU kg 0 0 0 0 0 0 0 0
MFR kg 0 0 0 0 0 9.16E+00 0 0
MER kg 0 0 0 0 0 0 0 0
EEE MJ 0 0 4.24E+01 0 0 0 0 0
4 Environmental Product Declaration - KONE - Sliding Door 50 / 50E / 50T / 50ET / 50L / 50 LT
EET MJ 0 0 9.73E+01 0 0 0 0 0
HWD = Hazardous waste disposed; NHWD = Non-hazardous waste disposed; RWD = Radioactive waste disposed; CRU = Components for re-use;
MFR = Materials for recycling; MER = Materials for energy recovery; EEE = Exported electrical energy; EET = Exported thermal energy
RESULTS OF THE LCA – additional impact categories according to EN 15804+A2-optional:
1 piece Sliding Door 50 / 50E / 50T / 50ET / 50L / 50 LT
Parameter Unit A1-A3 A4 A5 C1 C2 C3 C4 D
Disease
PM 2.1E-05 1.26E-08 5.2E-08 0 6.12E-09 4.38E-08 3.16E-07 -2.86E-06
incidence
IR kBq U235 eq 2.63E+01 5E-03 3.5E-02 0 3E-03 3E-02 5.5E-02 -1.74E+01
ETP-fw CTUe 8.57E+03 2.42E+01 3.98E+00 0 1.17E+01 3.36E+00 2.67E+01 -2.93E+02
HTP-c CTUh 2.66E-07 4.54E-10 3.45E-10 0 2.2E-10 2.91E-10 3.95E-09 -1.46E-08
HTP-nc CTUh 4.89E-06 1.94E-08 3.49E-08 0 9.41E-09 2.94E-08 4.35E-07 -4.32E-07
SQP SQP 4.19E+02 8.8E-02 3.18E+00 0 4.2E-02 2.68E+00 9.73E+00 -6.51E+01
PM = Potential incidence of disease due to PM emissions; IR = Potential Human exposure efficiency relative to U235; ETP-fw = Potential comparative
Toxic Unit for ecosystems; HTP-c = Potential comparative Toxic Unit for humans (cancerogenic); HTP-nc = Potential comparative Toxic Unit for humans
(not cancerogenic); SQP = Potential soil quality index
Disclaimer 1 – for the indicator “Potential Human exposure efficiency relative to U235”. This impact category deals mainly with the
eventual impact of low-dose ionizing radiation on human health of the nuclear fuel cycle. It does not consider effects due to possible
nuclear accidents, occupational exposure or radioactive waste disposal in underground facilities. Potential ionizing radiation from the
soil, radon and from some construction materials is also not measured by this indicator.
Disclaimer 2 – for the indicators “abiotic depletion potential for non-fossil resources”, “abiotic depletion potential for fossil resources”,
“water (user) deprivation potential, deprivation-weighted water consumption”, “potential comparative toxic unit for ecosystems”,
“potential comparative toxic unit for humans – cancerogenic”, “Potential comparative toxic unit for humans - not cancerogenic”,
“potential soil quality index”. The results of this environmental impact indicator shall be used with care as the uncertainties on these
results are high as there is limited experience with the indicator.
This EPD was created using a software tool.
References
DIN 18650-1 declarations — Type III environmental declarations —
DIN 18650-1:2010-06,Powered pedestrian doors –Part 1: Principles and procedures
Product requirements and test methods.
European Chemicals Agency (ECHA)
DIN 18650-2 https:echa.europa.eu/de/home
DIN 18650-2:2010-06, Powered pedestrian doors –Part 2:
Safety at powered pedestrian doors. GaBi ts software
Sphera Solutions GmbH Gabi Software System and Database
EN 15804 for Life CyclenEngineering 1992-2020 Version 10.0.0.71
EN 15804:2012-04, Sustainability of construction works – University of Stuttgart Leinfelden-Echterdingen
Environmental product declarations – Core rules for the product
category of construction products; German version EN GaBi ts documentation
15804:2012. GaBi life cycle inventory data documentation
(https://www.gabisoftware.com/support/gabi/gabidatabase-
EN 16005 2020-lci-documentation/).
EN 16005:2013-01, Power operated pedestrian doorsets -
Safety in use - Requirements and test methods; German IBU 2021
version EN 16005:2012 General Instructions for the EPD programme of Institut Bauen
und Umwelt e.V. Version 2.0, Berlin: Institut Bauen und Umwelt
EN 60335-1 e.V., 2021.
EN 60335-1; VDE 0700-1:2012-10:2012-10, Household and www.ibu-epd.com
similar electrical appliances – Safety - Part 1: General
requirements (IEC 60335-1:2010, modified); German version LCA-tool dormakaba
EN 60335-1:2012. LCA tool, ENS doors LCA tool no.: BU-DOR-202107-LT1-EN
Developed by Sphera Solutions GmbH.
EN 60335
EN 60335-2-103/A1; Household and similar electrical PCR Part A
appliances - Safety - Part 2-103: Particularrequirements for PCR – Part A: Calculation Rules for the Life Cycle Assessment
drives for gates, doors and windows (IEC 61/2863/CDV:2005); and Requirements on the Project Re-port according to EN
German version EN 60335-2-103:2003/prA1:2005.2011/65/EU 15804+A2:2019, Version 1.0, Institut Bauen und Umwelt e.V.,
www.ibu-epd.com.
ISO 13849-1
ISO 13849-1:2008-12, Safety of machinery – Safetyrelated PCR Part B
parts of control systems – Part 1: General principles for design PCR – Part B: Requirements on the EPD for Automatic doors,
(ISO 13849-1:2006. automatic gates, and revolving door systems, 08.2021, Institut
Bauen und Umwelt e.V.,
ISO 14025 www.ibu-epd.com.
DIN EN ISO 14025:201110, Environmental labels and
5 Environmental Product Declaration - KONE - Sliding Door 50 / 50E / 50T / 50ET / 50L / 50 LT
REACH Regulation
REACH Regulation (EC) No 1907/2006 of the European
Parliament and of the Council on the Registration, Evaluation,
Authorisation and Restriction of Chemicals.
ROHS3 Directive
Directive 2011/65/EU of the European Parliament and of the
Council of 8 June 2011 on the restriction of the use of certain
hazardous substances in electrical and electronic equipment
6 Environmental Product Declaration - KONE - Sliding Door 50 / 50E / 50T / 50ET / 50L / 50 LT
Publisher
Institut Bauen und Umwelt e.V. +49 (0)30 3087748- 0
Hegelplatz 1 info@ibu-epd.com
10117 Berlin www.ibu-epd.com
Germany
Programme holder
Institut Bauen und Umwelt e.V. +49 (0)30 3087748- 0
Hegelplatz 1 info@ibu-epd.com
10117 Berlin www.ibu-epd.com
Germany
Author of the Life Cycle Assessment
dormakaba International Holding GmbH +49 2333 793-0
DORMA Platz 1 info.de@dormakaba.com
58256 Ennepetal www.dormakaba.com
Germany
Owner of the Declaration
KONE Corporation +358(0)204 75 1
Keilasatama 3 contact@kone.com
02150 ESPOO www.kone.com
Finland
7 Environmental Product Declaration - KONE - Sliding Door 50 / 50E / 50T / 50ET / 50L / 50 LT
