ENVIRONMENTAL PRODUCT DECLARATION
as per ISO 14025 and EN 15804+A2
Owner of the Declaration danfloor a/s
Programme holder Institut Bauen und Umwelt e.V. (IBU)
Publisher Institut Bauen und Umwelt e.V. (IBU)
Declaration number EPD-DAN-20220312-CBA1-EN
Issue date 31.01.2023
Valid to 30.01.2028
Tufted wall-to-wall carpet
With a maximum total pile weight of 1275 g/m2, PP, SBR
based foam backing
danfloor a/s
www.ibu-epd.com | https://epd-online.com
Umwelt Produktdeklaration Name des Herstellers – Name des Produkts
General Information
danfloor a/s Tufted wall-to-wall carpet
With a maximum total pile weight of
1275 g/m2, PP, SBR based foam
backing
Programme holder Owner of the declaration
IBU – Institut Bauen und Umwelt e.V. danfloor a/s
Hegelplatz 1 Østerbro 9
10117 Berlin 6933 Kibæk
Germany Denmark
www.danfloor.com
Declaration number Declared product / declared unit
EPD-DAN-20220312-CBA1-EN 1 m² tufted wall-to-wall carpet, PP pile material with a
SBR based foam backing
This declaration is based on the product Scope:
category rules: The manufacturer declaration applies to tufted wall-to-
Floor coverings, 02/2018 wall carpet with a SBR based foam backing, a pile
(PCR checked and approved by the SVR) material of PP with a maximum total pile weight of
1275 g/m2. The products are produced in Kibæk,
Denmark and coated in Bording, Denmark.
Issue date
LCA results for products with a maximum total pile
31.01.2023
weight of 1030 g/m2 can be taken from the
corresponding tables of the annexe. Specific data for
Valid to every product within the declared group of products in
30.01.2028 relation to its total pile weight can be calculated by
using equation 1 given in the annexe (see annexe
chapter: 'General Information on the annexe'). The
declaration is only valid in conjunction with a valid
GUT-PRODIS license of the product.
The owner of the declaration shall be liable for the
underlying information and evidence; the IBU shall not
be liable with respect to manufacturer information, life
cycle assessment data and evidences.
The EPD was created according to the specifications
of EN 15804+A2. In the following, the standard will be
simplified as EN 15804.
Verification
The standard EN 15804 serves as the core PCR
Independent verification of the declaration and data
according to ISO 14025:2011
Dipl. Ing. Hans Peters internally x externally
(chairman of Institut Bauen und Umwelt e.V.)
Dr. Alexander Röder Angela Schindler
(Managing Director Institut Bauen und Umwelt e.V.)) (Independent verifier)
Product
Product description/Product definition Regulation (CPR) applies. The product needs a
The declaration applies to tufted wall-to wall carpet Declaration of Performance (DoP) taking into
having a surface pile of solution-dyed polypropylene consideration EN 14041:2018-05, Resilient, textile and
with a maximum total pile weight of 1275 g/m2. The laminate floor coverings - Essential characteristics, and
backing of the carpet consists of a SBR based foam the CE-marking. The DoP of the product can be found
backing. on the manufacturer's technical information section.
For the application and use of the product the
For the placing on the market of the specific product in respective national provisions apply.
the European Union/European Free Trade Association
(EU/EFTA) (with the exception of Switzerland) Application
Regulation (EU) No. 305/2011 Construction Product The use class of the specific product as defined in
2 Environmental Product Declaration danfloor – Tufted wall-to-wall carpet, polypropylene with a maximum total pile weight
of 1275 g/m2 and a foam backing
EN 1307 can be found in the Product Information
System (PRODIS) using the PRODIS registration The specific product coverd by the EPD contains
number of the product. substances listed in the ECHA candidate list
(08.07.2021) or other carcinogenic, mutagenic or
Technical Data reprotoxic (CMR) substances in categories 1A or 1B
which are not on the candidate list exceeding 0.1
percentage by mass: no
Constructional data according to EN 1307 The products are registered in the GUT-PRODIS
Name Value Unit Information System. The PRODIS system ensures
Product Form Wall-to-wall carpet on rolls - compliance with limitations of various chemicals and
Type of manufacture Tufted carpet - Volatile Organic Compounds (VOC)-emissions and a
Yarn type Polypropylene - ban on the use of all substances that are listed as
Secondary backing SBR based foam backing - 'Substances of Very High Concern' (SVHC) under
Total pile weight max. 1275 g/m² REACH.
Total carpet weight 3505 g/m2
Reference service life
The service life of textile floor coverings strongly
Performance data of the product in accordance with depends on the correct installation taking into account
the declaration of performance with respect to its the declared use classification and the adherence to
essential characteristics according to EN 14041: 2018- cleaning and maintenance instructions.
05, Resilient, textile and laminate floor coverings - A calculation of the reference service life according to
Essential characteristics. ISO 15686 is not possible.
Additional product properties in accordance with EN Alternatively, a reference service life of 10 years can
1307 can be found on the Product Information System be assumed, during which the functional and visual
PRODIS using the PRODIS registration number of the quality is guaranteed (BNB, Nutzungsdauer von
product (www.pro-dis.info) or on the manufacturer's Bauteilen). The technical service life can be
technical information section. significantly longer.
Base materials/Ancillary materials
Name Value Unit
Polypropylene 40.1 %
Polymer dispersion 18.4 %
Limestone 24.6 %
ATH 14.4 %
Additives 2.5 %
LCA: Calculation rules
Declared Unit A1-A3 Production:
Energy supply and production of the basic material,
processing of secondary material, auxiliary material,
Name Value Unit transport of the material to the manufacturing site,
Declared unit 1 m2 emissions, waste water treatment, packaging material
Grammage 3.505 kg/m2 and waste processing up to the landfill disposal of
The declared unit refers to 1 m2 produced textile floor residual waste (except radioactive waste). Benefits for
covering. The Output of module A5 'Assembly' is 1 m2 generated electricity and steam due to the incineration
installed textile floor covering. of production waste are aggregated.
The layer thickness of the specific product covered by Biogenic carbon that is stored in renewable material
the EPD can be found on the Product Information (packaging paper) is taken into account as well as the
System PRODIS using the PRODIS registration associated carbon dioxide uptake from the air from
number of the product (www.pro-dis.info) or on the which this biogenic carbon comes.
manufacturer's technical information section.
A4 Transport:
Transport of the packed textile floor covering
from factory gate to the place of installation.
System boundary
A5 Installation:
Type of EPD: Installation of the textile floor covering, processing of
Cradle-to-gate with options, module C1-C4, module D, installation waste and packaging waste up to the
and additional modules A4, A5, B1, B2. landfill disposal of residual waste (except radioactive
waste), the production of the amount of carpet that
System boundaries of modules A, B, C, D: occurs as installation waste including its transport to
Modules C3, C4 and D are indicated separately for the place of installation.
three end-of-life scenarios: Generated electricity and steam due to the incineration
1 - landfill disposal of waste are listed in the result table as exported
2 - municipal waste incineration energy.
3 - recovery in a cement plant Biogenic carbon that is stored in renewable materials
3 Environmental Product Declaration danfloor – Tufted wall-to-wall carpet, polypropylene with a maximum total pile weight
of 1275 g/m2 and a foam backing
in packaging paper is released as carbon dioxide C3 Waste processing:
emissions into the air at the end of life in module A5. C3-1: Landfill disposal needs no waste processing.
Preparation of the floor and auxiliary materials C3-2: Impact from waste incineration (plant with
(adhesives, fixing agents, PET connectors) are beyond R1>0.6), generated electricity and steam are listed in
the system boundaries and not taken into account. the result table as exported energy.
C3-3: Collection of the carpet waste for recovery in the
B1 Use: cement industry, waste processing (granulating),
Indoor emissions during the use stage. After the first transport to the cement plant, emissions from the
year, no product-related Volatile Organic Compound incineration.
(VOC) emissions are relevant due to known VOC
decay curves of the product. C4 Disposal
C4-1: Impact from landfill disposal,
B2 Maintenance: C4-2: The carpet waste leaves the system in
Cleaning of the textile floor covering for a period of 1 module C3-2,
year: C4-3: The pre-processed carpet waste leaves the
Vacuum cleaning – electricity supply system in module C3-3.
Wet cleaning – electricity, water consumption,
production of the cleaning agent, waste water D Recycling potential:
treatment. Calculated benefits result from materials exclusive
The declared values in this module have to be secondary materials (net materials).
multiplied by the assumed service life of the floor D-A5: Benefits for generated energy due
covering in the building in question. to incineration of packaging and installation waste
(incineration plant with R1 > 0.6),
B3 - B5: D-1: Benefits for generated energy due to landfill
The modules are not relevant within the assumed disposal of carpet waste at the end-of-life,
reference service life of 10 years. D-2: Benefits for generated energy due to incineration
of carpet waste at the end-of-life (incineration plant
B6 - B7: with R1 > 0.6),
No energy and water input are required for the D-3: Benefits for saved fossil energy and saved
operation of the carpet in the use stage. The modules inorganic material due to recovery of the carpet in a
are not relevant and not declared. cement plant.
C1 De-construction: Comparability
The floor covering is de-constructed manually and no Basically, a comparison or an evaluation of EPD data
additional environmental impact is caused. is only possible if all the data sets to be compared
were created according to EN 15804 and the building
C2 Transport: context, respectively the product-specific
Transport of the carpet waste to a landfill, to the characteristics of performance, are taken into account.
municipal waste incineration plant (MWI) or to the
waste collection facility for recycling. Background data are taken from the GaBi database,
2022-1. Remaining data gaps are covered by the
ecoinvent 3.7 database, 2020.
LCA: Scenarios and additional technical information
Characteristic product properties Polyethylene packaging waste and installation waste
Information on biogenic carbon are considered to be incinerated in a municipal waste
incineration plant. Cardboard packaging waste is going
to be recycled.
Name Value Unit Preparation of the floor and auxiliaries (adhesives,
Biogenic carbon content in fixing agents, PET connectors etc.) are not taken into
accompanying packaging at 0.022 kg C account.
factory gate
1 kg biogenic Carbon is equivalent to 44/12 kg of CO Maintenance (B2)
2
The values for cleaning refer to 1 m2 floor covering per
year.
Depending on the application based on ISO 10874, the
Transport to the construction site (A4) technical service life recommended by the
Name Value Unit manufacturer and the anticipated strain on the floor by
Litres of fuel (truck, EURO 0-6 customers, the case-specific useful life can be
0.0082 l/100km
mix) established. Based on this useful life the effects of
Transport distance 700 km module B2 need to be calculated in order to obtain the
Capacity utilisation (including overall environmental impacts.
55 %
empty runs)
Installation in the building (A5)
Name Value Unit
Material loss 0.315 kg
4 Environmental Product Declaration danfloor – Tufted wall-to-wall carpet, polypropylene with a maximum total pile weight
of 1275 g/m2 and a foam backing
Name Value Unit
Maintenance cycle (vacuum Number
208
cleaning) /year
Number
Maintenance cycle (wet cleaning) 1,5
/year
Water consumption (wet cleaning) 0.004 m3
Cleaning agent (wet cleaning) 0.09 kg
Electricity consumption 0.314 kWh
For further information on cleaning and maintenance
see www.danfloor.com
Service life
Name Value Unit
Life Span (according to
10 a
BBSR)
Declared product Corresponds to the
properties (at the gate) and specifications of EN -
finishes 1307
An assumed quality of
Conforms to the
work, when installed in
manufacturer's -
accordance with the
instructions
manufacturer’s instructions
Usage conditions, e.g. Use in areas defined by
frequency of use, the use class according -
mechanical exposure to EN 1307
Maintenance e.g. required
According to the
frequency, type and quality
manufacturers -
and replacement of
instructions
components
End of Life (C1-C4)
Three different end-of-life scenarios are declared and
the results are indicated separately in module C.
Each scenario is calculated as a 100% scenario.
Scenario 1: 100 % landfill disposal
Scenario 2: 100 % municipal waste incineration (MWI)
with R1>0.6
Scenario 3: 100 % recovery in the cement industry
If combinations of these scenarios have to be
calculated this should be done according to the
following scheme:
EOL-impact = x % impact (Scenario 1)
+ y % impact (Scenario 2)
+ z % impact (Scenario 3)
with x % + y % + z % = 100 %
Name Value Unit
Collected as mixed construction
3.505 kg
waste (scenarios 1 and 2)
Collected separately (scenario 3) 3.505 kg
Landfilling (scenario 1) 3.505 kg
Energy recovery (scenario 2) 3.505 kg
Energy recovery (scenario 3) 2.138 kg
Recycling (scenario 3) 1.367 kg
Reuse, recovery and/or recycling potentials (D),
relevant scenario information
Recovery or recycling potentials due to the three end-
of-life scenarios (module C) are indicated separately.
Recycling in the cement industry (scenario 3)
The organic material of the carpet is used as an
alternative fuel in a cement kiln. It mainly substitutes
for lignite (68.8 %), hard coal (23.6 %) and petrol coke
(7.6 %). The inorganic material is substantially
integrated into the cement clinker and substitutes for
original material input. VDZ e.V.
5 Environmental Product Declaration danfloor – Tufted wall-to-wall carpet, polypropylene with a maximum total pile weight
of 1275 g/m2 and a foam backing
LCA: Results
The LCA results refer to all declared products with a maximum total pile weight of 1275 g/m2.
LCA results for products with a maximum total pile weight of 1030 g/m2 can be taken from the corresponding
tables of the annexe. Results for specific products with any other total pile weight can be calculated by using
equation 1 given in the annexe (see annexe chapter: 'General Information on the annexe').
The declared result figures in module B2 have to be multiplied by the assumed service life (in years) of the floor
covering in the building under consideration.
Information on non-relevant modules:
Modules B3 - B7 are not relevant during the service life of the carpet. Modules C3/1, C4/2 and C4/3 cause no
additional impact (see chapter "LCA: Calculation rules" in this document). Module C2 represents the transport for
scenarios 1, 2 and 3. Column D represents module D/A5.
DESCRIPTION OF THE SYSTEM BOUNDARY (X = INCLUDED IN LCA; ND = MODULE OR INDICATOR NOT
DECLARED; MNR = MODULE NOT RELEVANT)
BENEFITS AND
CONSTRUCTI LOADS
PRODUCT STAGE ON PROCESS USE STAGE END OF LIFE STAGE BEYOND THE
STAGE SYSTEM
BOUNDARIES
6 Environmental Product Declaration danfloor – Tufted wall-to-wall carpet, polypropylene with a maximum total pile weight
of 1275 g/m2 and a foam backing
lairetam
waR
ylppus tropsnarT
gnirutcafunaM
eht
morf
tropsnarT
etis
eht
ot
etag
ylbmessA esU
ecnanetniaM
riapeR
tnemecalpeR tnemhsibrufeR
ygrene
lanoitarepO esu
retaw
lanoitarepO esu
noitcurtsnoc-eD
noitilomed tropsnarT
gnissecorp
etsaW
lasopsiD -esueR -yrevoceR -gnilcyceR laitnetop
A1 A2 A3 A4 A5 B1 B2 B3 B4 B5 B6 B7 C1 C2 C3 C4 D
X X X X X X X MNR MNR MNR ND ND X X X X X
RESULTS OF THE LCA - ENVIRONMENTAL IMPACT according to EN 15804+A2: 1 m² floor covering
Core Indicator Unit A1-A3 A4 A5 B1 B2 C1 C2 C3/2 C3/3 C4/1 D D/1 D/2 D/3
-
GWP-total [kg CO2-Eq.] 7.50E+02.12E-11.33E+00.00E+04.16E-10.00E+01.19E-25.77E+05.82E+02.49E-1-2.17E-10.00E+0 2.24E+0-5.86E-1
-
GWP-fossil [kg CO2-Eq.] 7.53E+02.08E-11.25E+00.00E+02.15E-10.00E+01.17E-25.77E+05.82E+02.48E-1-2.16E-10.00E+0 2.23E+0-5.85E-1
GWP-biogenic [kg CO2-Eq.] -3.00E-22.69E-3 7.76E-20.00E+04.16E-30.00E+01.51E-4 4.11E-4 9.50E-40.00E+0-1.10E-30.00E+0-1.14E-2-8.22E-4
GWP-luluc [kg CO2-Eq.] 3.36E-3 1.18E-3 4.27E-40.00E+01.96E-10.00E+06.61E-5 1.48E-4 3.17E-4 1.21E-4-2.37E-50.00E+0-2.44E-4-2.84E-4
3.10E- 1.27E- 2.82E- 7.11E- 3.42E- 6.07E- 3.34E- -1.46E- -1.50E- -8.16E-
ODP [kg CFC11-Eq.] 0.00E+03.42E-80.00E+0 0.00E+0
11 14 12 16 13 13 13 12 11 13
AP [mol H+-Eq.] 1.61E-2 1.26E-3 1.68E-30.00E+08.32E-40.00E+07.06E-5 1.19E-3 1.40E-3 7.36E-4-2.84E-40.00E+0-2.92E-3-2.17E-3
EP-freshwater [kg P-Eq.] 2.06E-5 6.30E-7 1.96E-60.00E+05.19E-60.00E+03.54E-8 5.36E-7 6.77E-7 4.64E-5-2.96E-70.00E+0-3.05E-6-6.50E-7
EP-marine [kg N-Eq.] 4.74E-3 6.17E-4 5.21E-40.00E+01.97E-40.00E+03.47E-5 3.89E-4 4.85E-4 1.63E-4-7.71E-50.00E+0-7.94E-4-6.64E-4
EP-terrestrial [mol N-Eq.] 5.09E-2 6.83E-3 5.73E-30.00E+02.83E-30.00E+03.84E-4 5.38E-3 6.43E-3 1.79E-3-8.26E-40.00E+0-8.50E-3-7.28E-3
POCP [kg NMVOC-Eq.]1.49E-2 1.17E-3 1.54E-3 4.18E-4 9.83E-40.00E+06.56E-5 1.06E-3 1.24E-3 5.24E-4-2.16E-40.00E+0-2.22E-3-1.99E-3
9.92E-
ADPE [kg Sb-Eq.] 1.46E-6 1.77E-8 1.35E-70.00E+02.30E-70.00E+0 1.67E-8 2.41E-8 1.72E-8-3.25E-80.00E+0-3.35E-7-5.64E-8
10
- - -
ADPF [MJ] 2.08E+22.82E+01.92E+10.00E+05.90E+00.00E+01.59E-11.82E+02.55E+03.53E+0 0.00E+0
3.68E+0 3.79E+17.08E+1
[m³ world-Eq
WDP 8.15E-1 1.89E-3 1.38E-10.00E+09.99E-20.00E+01.06E-4 6.81E-1 6.85E-1-2.64E-3-2.27E-20.00E+0-2.34E-1-8.58E-2
deprived]
GWP = Global warming potential; ODP = Depletion potential of the stratospheric ozone layer; AP = Acidification potential of land and water; EP =
Caption Eutrophication potential; POCP = Formation potential of tropospheric ozone photochemical oxidants; ADPE = Abiotic depletion potential for non-
fossil resources; ADPF = Abiotic depletion potential for fossil resources; WDP = Water (user) deprivation potential
RESULTS OF THE LCA - INDICATORS TO DESCRIBE RESOURCE USE according to EN 15804+A2: 1 m²
floor covering
Indicator Unit A1-A3 A4 A5 B1 B2 C1 C2 C3/2 C3/3 C4/1 D D/1 D/2 D/3
PERE [MJ] 2.76E+1 1.60E-1 2.64E+0 0.00E+0 3.69E+0 0.00E+0 9.01E-3 3.73E-1 5.76E-1 2.90E-1 -1.01E+0 0.00E+0 -1.04E+1-8.25E-1
PERM [MJ] 9.70E-2 0.00E+0 -9.70E-2 0.00E+0 0.00E+0 0.00E+0 0.00E+0 0.00E+0 0.00E+0 0.00E+0 0.00E+0 0.00E+0 0.00E+0 0.00E+0
PERT [MJ] 2.77E+1 1.60E-1 2.55E+0 0.00E+0 3.69E+0 0.00E+0 9.01E-3 3.73E-1 5.76E-1 2.90E-1 -1.01E+0 0.00E+0 -1.04E+1-8.25E-1
PENRE [MJ] 1.30E+2 2.83E+0 1.97E+1 0.00E+0 5.90E+0 0.00E+0 1.59E-1 7.96E+1 8.04E+1 3.53E+0 -3.68E+0 0.00E+0 -3.79E+1-7.09E+1
PENRM [MJ] 7.83E+1 0.00E+0 -4.60E-1 0.00E+0 0.00E+0 0.00E+0 0.00E+0 -7.78E+1-7.78E+1 0.00E+0 0.00E+0 0.00E+0 0.00E+0 0.00E+0
PENRT [MJ] 2.09E+2 2.83E+0 1.92E+1 0.00E+0 5.90E+0 0.00E+0 1.59E-1 1.82E+0 2.55E+0 3.53E+0 -3.68E+0 0.00E+0 -3.79E+1-7.09E+1
SM [kg] 4.34E-2 0.00E+0 3.91E-3 0.00E+0 0.00E+0 0.00E+0 0.00E+0 0.00E+0 0.00E+0 0.00E+0 0.00E+0 0.00E+0 0.00E+0 8.10E-1
RSF [MJ] 0.00E+0 0.00E+0 0.00E+0 0.00E+0 0.00E+0 0.00E+0 0.00E+0 0.00E+0 0.00E+0 0.00E+0 0.00E+0 0.00E+0 0.00E+0 0.00E+0
NRSF [MJ] 0.00E+0 0.00E+0 0.00E+0 0.00E+0 0.00E+0 0.00E+0 0.00E+0 0.00E+0 0.00E+0 0.00E+0 0.00E+0 0.00E+0 0.00E+0 0.00E+0
FW [m³] 3.87E-2 1.81E-4 5.01E-3 0.00E+0 3.34E-3 0.00E+0 1.02E-5 1.60E-2 1.62E-2 4.13E-5 -9.62E-4 0.00E+0 -9.90E-3 -6.57E-3
PERE = Use of renewable primary energy excluding renewable primary energy resources used as raw materials; PERM = Use of
renewable primary energy resources used as raw materials; PERT = Total use of renewable primary energy resources; PENRE = Use of
non-renewable primary energy excluding non-renewable primary energy resources used as raw materials; PENRM = Use of non-
Caption
renewable primary energy resources used as raw materials; PENRT = Total use of non-renewable primary energy resources; SM = Use
of secondary material; RSF = Use of renewable secondary fuels; NRSF = Use of non-renewable secondary fuels; FW = Use of net fresh
water
RESULTS OF THE LCA – WASTE CATEGORIES AND OUTPUT FLOWS according to EN 15804+A2:
1 m² floor covering
Indicator Unit A1-A3 A4 A5 B1 B2 C1 C2 C3/2 C3/3 C4/1 D D/1 D/2 D/3
HWD [kg] 3.43E-8 1.35E-11 3.11E-9 0.00E+0 4.19E-5 0.00E+0 7.61E-132.25E-102.55E-105.44E-10-4.99E-100.00E+0 -5.14E-9-4.34E-10
NHWD [kg] 3.58E-1 4.05E-4 1.01E-1 0.00E+0 7.30E-3 0.00E+0 2.28E-5 7.59E-1 7.60E-1 3.49E+0 -1.85E-3 0.00E+0 -1.91E-2 -2.42E-1
RWD [kg] 4.76E-3 3.48E-6 4.37E-4 0.00E+0 3.76E-4 0.00E+0 1.96E-7 8.55E-5 1.38E-4 4.33E-5 -2.89E-4 0.00E+0 -2.97E-3 -1.77E-4
CRU [kg] 0.00E+0 0.00E+0 0.00E+0 0.00E+0 0.00E+0 0.00E+0 0.00E+0 0.00E+0 0.00E+0 0.00E+0 0.00E+0 0.00E+0 0.00E+0 0.00E+0
MFR [kg] 3.31E-2 0.00E+0 5.29E-2 0.00E+0 0.00E+0 0.00E+0 0.00E+0 0.00E+0 8.10E-1 0.00E+0 0.00E+0 0.00E+0 0.00E+0 0.00E+0
MER [kg] 0.00E+0 0.00E+0 0.00E+0 0.00E+0 0.00E+0 0.00E+0 0.00E+0 0.00E+0 0.00E+0 0.00E+0 0.00E+0 0.00E+0 0.00E+0 0.00E+0
EEE [MJ] 0.00E+0 0.00E+0 9.69E-1 0.00E+0 0.00E+0 0.00E+0 0.00E+0 9.97E+0 0.00E+0 0.00E+0 0.00E+0 0.00E+0 0.00E+0 0.00E+0
EET [MJ] 0.00E+0 0.00E+0 1.75E+0 0.00E+0 0.00E+0 0.00E+0 0.00E+0 1.81E+1 7.78E+1 0.00E+0 0.00E+0 0.00E+0 0.00E+0 0.00E+0
HWD = Hazardous waste disposed; NHWD = Non-hazardous waste disposed; RWD = Radioactive waste disposed; CRU = Components
Caption for re-use; MFR = Materials for recycling; MER = Materials for energy recovery; EEE = Exported electrical energy; EET = Exported
thermal energy
RESULTS OF THE LCA – additional impact categories according to EN 15804+A2-optional:
1 m² floor covering
Indicator Unit A1-A3 A4 A5 B1 B2 C1 C2 C3/2 C3/3 C4/1 D D/1 D/2 D/3
[Disease
PM 1.61E-7 7.26E-9 1.63E-8 0.00E+0 6.84E-8 0.00E+04.08E-10 1.18E-8 1.32E-8 7.08E-9 -2.35E-9 0.00E+0 0.00E+0 -3.66E-8
Incidence]
[kBq U235-
IRP 7.66E-1 5.11E-4 7.02E-2 0.00E+0 6.78E-2 0.00E+0 2.87E-5 1.33E-2 2.22E-2 6.39E-3 -4.89E-2 0.00E+0 0.00E+0 -2.05E-2
Eq.]
ETP-fw [CTUe] 9.66E+1 1.96E+0 8.98E+0 3.60E-3 2.69E+0 0.00E+0 1.10E-1 1.08E+0 1.50E+0 3.45E+0 -8.04E-1 0.00E+0 0.00E+0-1.27E+1
-3.71E- -1.56E-
HTP-c [CTUh] 3.27E-9 3.96E-113.04E-100.00E+06.21E-100.00E+02.22E-126.65E-117.61E-111.55E-10 0.00E+0 0.00E+0
11 10
HTP-nc [CTUh] 2.03E-7 2.35E-9 1.89E-8 2.60E-11 9.46E-9 0.00E+01.32E-10 4.16E-9 4.64E-9 1.30E-8 -1.42E-9 0.00E+0 0.00E+0 -9.51E-9
SQP [-] ND ND ND ND ND ND ND ND ND ND ND ND ND ND
PM = Potential incidence of disease due to PM emissions; IR = Potential Human exposure efficiency relative to U235; ETP-fw = Potential
Caption comparative Toxic Unit for ecosystems; HTP-c = Potential comparative Toxic Unit for humans (cancerogenic); HTP-nc = Potential
comparative Toxic Unit for humans (not cancerogenic); SQP = Potential soil quality index
The SQP indicator is not given due to considerable uncertainties in the calculation.
The result figures given in module B2 refer to a period of 1 year because a reference service life is not declared.
They have to be multiplied by the assumed service life (in years) of the floor covering in the building under
consideration.
Disclaimer 1 – for the indicator “Potential Human exposure efficiency relative to U235”.
This impact category deals mainly with the eventual impact of low dose ionizing radiation on human health of the
nuclear fuel cycle. It does not consider effects due to possible nuclear accidents, occupational exposure or
radioactive waste disposal in underground facilities. Potential ionizing radiation from the soil, from radon and from
some construction materials is also not measured by this indicator.
Disclaimer 2 – for the indicators “abiotic depletion potential for non-fossil resources”, “abiotic depletion potential
for fossil resources”, “water (user) deprivation potential, deprivation-weighted water consumption”, “potential
comparative toxic unit for ecosystems”, “potential comparative toxic unit for humans – cancerogenic”, “Potential
comparative toxic unit for humans - not cancerogenic”, “potential soil quality index”.
The results of this environmental impact indicator shall be used with care as the uncertainties on these results are
high or as there is limited experience with the indicator.
References
EN 1307 floor coverings – Environmental product declarations –
DIN EN 1307: 2014+A1:2016+A2:2018-05: Textile Product category rules
floor coverings - Classification
ISO 10874
EN 13501-1 DIN EN ISO 10874: 2012+A1:2021-04: Resilient,
DIN EN 13501-1:2019-05: Fire classification of textile and laminate floor coverings - Classification
construction products and building elements - Part 1:
Classification using data from reaction to fire tests ISO 14025
DIN EN /ISO 14025:2011-10/, Environmental labels
EN 14041 and declarations — Type III environmental
DIN EN 14041: 2018-05 and DIN EN 14041: 2008-05: declarations — Principles and procedures
Resilient, textile and laminate floor coverings -
Essential characteristics ISO 14040
DIN EN ISO 14040:2006+A1:2020 Environmental
EN 15804 management - Life cycle assessment - Principles and
DIN EN 15804:2012+A2:2019+AC:2021, Sustainability framework
of construction works — Environmental Product
Declarations — Core rules for the product category of
construction products
ISO 14044
EN 16810 DIN EN ISO 14044:2006+A1:2018+A2:2020
DIN EN 16810: 2017-08: Resilient, textile and laminate Environmental management - Life cycle assessment -
Requirements and guidelines
7 Environmental Product Declaration danfloor – Tufted wall-to-wall carpet, polypropylene with a maximum total pile weight
of 1275 g/m2 and a foam backing
GaBi database
ISO 15686 GaBi Software-System and Database for Life Cycle
ISO 15686: Buildings and constructed assets - Engineering, thinkstep AG, Leinfelden-Echterdingen,
Service life planning 2022-1
ISO 15686-1: 2011-05: Part 1: General principles and
framework PCR Part A
ISO 15686-2: 2012-05: Part 2: Service life prediction Product Category Rules for Building-Related Products
procedures and Services Part A: Calculation Rules for the Life
ISO 15686-7: 2017-04: Part 7: Performance Cycle Assessment and Requirements on the Project
evaluation for feedback of service life data Report according to EN 15804+A2:2019, V1.1, Berlin:
from practice Institut Bauen und Umwelt e.V. (IBU), January 2021
ISO 15686-8: 2008-06: Part 8: Reference service life
and service-life estimation PCR Part B
Product Category Rules for Building-Related Products
Regulation (EU) No. 305/2011 and Services
Regulation No. 305/2011 Construction Products Part B: Requirements on the EPD for floor coverings,
Regulation (CPR) of the European Council and of the V1.2, Berlin: Institut Bauen und Umwelt e.V. (IBU),
European Parliament, April 2011 February 2018
General Instructions for the IBU-EPD Program PRODIS
General Instructions for the EPD-Program of the Product Information System (PRODIS) of the
Institut Bauen und Umwelt e.V., The Preparation of European Carpet Industry, Gemeinschaft
Environmental Product Declarations - EPDs, version umweltfreundlicher Teppichboden e.V (GUT) and
2.0, Institut Bauen und Umwelt e.V., Berlin, January European Carpet and Rug Association
2021, www.ibu-epd.de (ECRA), http://www.pro-dis.info
BNB, Nutzungsdauer von Bauteilen REACH
Bewertungssystem Nachhaltiges Bauen (BNB), Regulation (EC) No 1907/2006 of the European
Nutzungsdauer von Bauteilen, Bundesministerium des Parliament and of the Council of 18 December 2006
Inneren, für Bau und Heimat, 24.02.2017 concerning the Registration, Evaluation, Authorisation
and Restriction of Chemicals (REACH), June 2017,
ECHA candidate list last update: 08.07.2021
Candidate List of substances of very high concern
(SVHCs) for authorisation, 08.07.2021, European VDZ e.V.
Chemicals Agency (ECHA), Helsinki, Finland Association of German Cement Works, Ed. Environ-
mental Data of the German Cement Industry 2020
ecoinvent
ecoinvent, Zurich, Switzerland, database version 3.7,
published September 2020
8 Environmental Product Declaration danfloor – Tufted wall-to-wall carpet, polypropylene with a maximum total pile weight
of 1275 g/m2 and a foam backing
Publisher
Institut Bauen und Umwelt e.V. Tel +49 (0)30 3087748- 0
Hegelplatz 1 Fax +49 (0)30 3087748- 29
10117 Berlin Mail info@ibu-epd.com
Germany Web www.ibu-epd.com
Programme holder
Institut Bauen und Umwelt e.V. Tel +49 (0)30 - 3087748- 0
Hegelplatz 1 Fax +49 (0)30 – 3087748 - 29
10117 Berlin Mail info@ibu-epd.com
Germany Web www.ibu-epd.com
Author of the Life Cycle
Assessment Tel +49 (0)241 96843 410
Gemeinschaft umweltfreundlicher Fax +49 (0)241 96843 400
Teppichboden (GUT) e.V. Mail mail@gut-ev.de
Schönebergstraße 2 Web www.gut-ev.org
52068 Aachen
Germany
Owner of the Declaration
danfloor a/s Tel +4596991900
Østerbro 9 Fax +4596991999
6933 Kibæk Mail sales@danfloor.com
Denmark Web www.danfloor.com
