ENVIRONMENTAL-PRODUCT DECLARATION
as per ISO 14025 and EN 15804+A2
Owner of the Declaration dormakaba International Holding GmbH
Publisher Institut Bauen und Umwelt e.V. (IBU)
Programme holder Institut Bauen und Umwelt e.V. (IBU)
Declaration number EPD-DOR-20210182-CBA2-EN
Issue date 01/10/2021
Valid to 30/09/2026
Reversible Double Cylinder - penta, quattro, gemini, expert, matrix
dormakaba
www.ibu-epd.com | https://epd-online.com
General Information
dormakaba Reversible Double Cylinder - penta, quattro,
gemini, expert, matrix
Programme holder Owner of the declaration
IBU – Institut Bauen und Umwelt e.V. dormakaba International Holding GmbH
Hegelplatz 1 DORMA Platz 1
10117 Berlin 58256 Ennepetal
Germany Germany
Declaration number Declared product / declared unit
EPD-DOR-20210182-CBA2-EN 1 piece of the product: one (1) dormakaba expert mechanical key system,
consisting of the following items:
- one (1) expert plus (K83) double cylinder
- three (3) expert plus (K83) reversible keys
- one (1) cylinder mounting screw
- one (1) security card
- one (1) user manual
- packaging material
This declaration is based on the product category rules: Scope:
Building Hardware products, 01/08/2021 This EPD is a specific product declaration for the expert plus (K83) double
(PCR checked and approved by the SVR) cylinder including three keys. It is also representative for the systems
penta,quattro, gemini and matrix. The underlying life cycle assessment is
based on the entire life cycle of this specific mechanical key system. The
Issue date products are manufactured at the dormakaba production facilities in
Eggenburg (Austria). Green Electricity is beeing used at the production
01/10/2021
site.
Data represents the year 2021.
Valid to
The owner of the declaration shall be liable for the underlying information
30/09/2026 and evidence; the IBU shall not be liable with respect to manufacturer
information, life cycle assessment data and evidences.
The EPD was created according to the specifications of EN 15804+A2. In
the following, the standard will be simplified as EN 15804 bezeichnet.
Verification
The standard EN 15804 serves as the core PCR
Independent verification of the declaration and data according to ISO
14025:2011
internally X externally
Dipl.-Ing Hans Peters
(chairman of Institut Bauen und Umwelt e.V.)
Florian Pronold Dr.-Ing. Wolfram Trinius,
(Managing Director Institut Bauen und Umwelt e.V.) (Independent verifier)
1 Environmental-Product Declaration - dormakaba - Reversible Double Cylinder - penta, quattro, gemini, expert, matrix
Product
• quattro and expert have 4 pin rows with up to 22
Product description/Product definition simultaneously used pin positions out of 44 positions in
Information about the enterprise total
dormakaba stands for a broad offering of products, solutions • gemini and matrix have 3 pin rows with 16
and services for smart and secure access to buildings and simultaneously used pin positions out of 32 positions in
rooms from a single source. total
• cylinder bodies are made of brass
Product description/ Product definition • keys are made of nickel silver
penta cross (K90), penta (K84), quattro plus (K85), gemini plus Please list the Technical Data according to the
(K87), expert cross (K89), expert plus (K83) and matrix plus List in the chapter “Product group specific calculation rules”
(K86) are patented, reversible master key systems representing
the premium segment. The patent offers legal protection
against commercial imitation. Duplicate keys are only made by
dormakaba itself or by authorized partners and require Example:
identification by means of a security card.
While penta, quattro and gemini are in-house systems that are
exclusively manufactured in our factories, expert and matrix are
partner systems that can also be assembled by authorized Technical
dealers. Data for Locking Cylinders acc. to the classification in EN
For placing the mechanical key systems on the market in the 1303: Delivery status:
European Union/European Free Trade Association (EU/EFTA, One (1) serial standard double cylinder includes three (3) keys,
with the exception of Switzerland) the following legal provisions a mounting-screw, a user-manual and a security card. Including
apply: the packaging the cylinder will be supplied with a weight of
All systems are classified according to the European locking 0,270kg.
cylinder standards EN1303 and DIN18252. While the basic
cylinder configuration already fulfils the attack resistance class Base materials/Ancillary materials
B, the highest protection grade D can be achieved with The material composition
integrated carbide steel inserts. of the product is the following:
dormakaba mechanical cylinders fulfill the material
requirements given within the Directive RoHS 2011/65/EU. In
addition, cylinders are fire protection tested according to EN
1634-1 and EN 1634-2.
These figures are also
representative for the systems penta, quattro, gemini and
matrix.
The cylindersand keys contain partial articles which contain
One speciality about the penta, quattro gemini, expert and
substances
matrix design is the insert modularity. This guarantees a
listed in the Candidate List of REACH Regulation
maximum on flexibility as the interchangeable inserts can be
1907/2006/EC (date:19.01.2021) exceeding 0.1 percentage by
used in different housing length as well as in all cylinder types
mass: yes
(e.g. double-, single-, thumbturn cylinders, rim, padlocks,
camlocks etc.) For placing the mechanical key systems on the • Lead (Pb): 7439-92-1 (CAS-No.)
market in the European Union/European Free Trade is included in some of the alloys used. The
Association (EU/EFTA, with the exception of Switzerland) the concentration of lead in each
following legal provisions apply: individual alloy does not exceed 4.0% (by mass).
· DIN EN 1303: 2015-08
· DIN 18252: 2018-05 The candidate list can be found on the /ECHA/ website
· RoHS 2011/65/EU address: https://echa.europa.eu/de/home
Application Environment and health during use
The dormakaba reversible cylinder range with penta, quattro,
Reference service life
gemini, expert and matrix can be used in both residential as
well as in the commercial segment in small and simple as well The
as in large and complex applications, thanks to its versatility. life cycle (security and function) of a lock cylinder is about 10-
Nearly limitless application options are possible. 15 years,
depending on the application and frequency of use. The
Technical Data cylinders are tested to 100,000
locking cycles minimum (EN1303:2015-08). This corresponds
• penta has 5 pin rows with up to 22 simultaneously used
to approximately
pin positions out of 85 positions in total
15-18 locking cycles per day for 15 years.
LCA: Calculation rules
2 Environmental-Product Declaration - dormakaba - Reversible Double Cylinder - penta, quattro, gemini, expert, matrix
Construction stage - Modules A4-A5
Declared Unit The construction process stage includes:
The declared unit is 1 piece of the product: expert — A4, transport to the building site;
Declared unit — A5, installation into the building;
including provision of all materials, products and
Name Value Unit
energy, as well as waste processing up to the end-ofwaste
Declared unit 1 piece/product
state or disposal of final residues during the
Conversion factor to 1 kg (kg/piece) 0.27 - construction process stage.
Mass of declared product including
0.27 kg
packaging
End-of-life stage– Modules C1-C4 and D
For IBU core EPDs (where clause 3.6 is part of the EPD): for
The end-of-life stage includes:
average EPDs, an estimate of the robustness of the LCA
— C1, de-construction, demolition:
values must be made, e.g. concerning variability of the
— C2, transport to waste processing;
production process, geographical representativeness and the
— C3, waste processing for reuse, recovery and/or
influence of background data and preliminary products
recycling;
compared to the environmental impacts caused by actual
— C4, disposal;
production.
including provision and all transport, provision of all
materials, products and related energy and water use.
System boundary Module D (Benefits and loads beyond the system
boundary) includes:
The type of EPD is according to EN 15804:
— D, recycling potentials, expressed as net impacts
"cradle to gate with options, modules C1–C4, and module D".
and benefits.
The
following modules are declared: A1-A3, C1-C4, D and
Geographic Representativeness
additional modules: A4 + A5
Land or region, in which the declared product system is
Production - Module A1-A3
manufactured, used or handled at the end of the product´s
The product stage includes:
lifespan: Austria
— A1, raw material extraction, processing and
mechanical treatments, processing of secondary
material input (e.g. recycling processes), Comparability
— A2, transport to the manufacturer,
Basically, a comparison or an evaluation of EPD data is only
— A3, manufacturing and assembly
possible if all the data sets to be compared were created
including provision of all materials, products and
according to EN 15804 and the building context, respectively
energy, as well as waste processing up to the end-of
the product-specific characteristics of performance, are taken
waste state.
into account. Background database: GaBi, SP40.
LCA: Scenarios and additional technical information
Characteristic product properties Name Value Unit
Information on biogenic carbon
Litres of fuel (per piece) 0.0015l/100km
Transport distance (plane) 80 km
The biogenic carbon content quantifies the amount of biogenic
carbon in a construction product leaving the factory gate, and it Transport distance (truck) 909 km
shall be separately declared for the product and for any Capacity utilisation (including empty runs)
51 %
accompanying packaging. average
If the total mass of biogenic carbon containing materials is less
Numbers reflect the average transport distances per cylinder.
than 5 % of the total mass of the product and accompanying
packaging, the declaration of biogenic carbon content may be
Installation into the building (A5)
omitted. The mass of packaging containing biogenic carbon
shall always be declared. Name Value Unit
Waste packaging (paper) 0,03328 kg
Note: 1 kg of biogenic carbon is equivalent to 44/12 kg of CO2.
In case a reference service life according to applicable ISO
Information on describing the biogenic Carbon Content at
standards is declared then the assumptions and in-use
factory gate
conditions underlying the determined RSL shall be declared. In
Name ValueUnit addition, it shall be stated that the RSL applies for the reference
Biogenic carbon content in accompanying kg conditions only.
0.01
packaging C
The same holds for a service life declared by the manufacturer.
Corresponding information related to in-use conditions needs
The following technical scenario information is required for the
not be provided if a service life taken from the list on service life
declared modules.
by BNB is declared.
Transport to the building site (A4)
End of life (C1-C4)
C1: The product dismantling from the building is done manually
without environmental burden.
3 Environmental-Product Declaration - dormakaba - Reversible Double Cylinder - penta, quattro, gemini, expert, matrix
Name Value Unit components are assumed to be incinerated with energy
recovery.
Collected separately waste type 0.237 kg
Recycling 0.231 kg
Reuse, recovery and/or recycling potentials (D),
Energy recovery 0.0062 kg
relevant scenario information
The product is disassembled in a recycling process. Collection rate is 100%.
Material recycling is then assumed for the metals. The plastic
4 Environmental-Product Declaration - dormakaba - Reversible Double Cylinder - penta, quattro, gemini, expert, matrix
LCA: Results
In Table 1 "Description of the system boundary", all declared modules shall be indicated with an "X"; all modules that are not declared
shall be indicated with "MND" (As default the modules B3, B4, B5 are marked as MNR – module not relevant). In the following tables,
columns can be deleted for modules that are not declared. Indicator values should be declared with three valid digits (eventually using
exponential form (e.g. 1,23E-5 = 0,0000123). A uniform format should be used for all values of one indicator.
If several modules are not declared and therefore have been deleted from the table, the abbreviations for the indicators can be
replaced by the complete names, while the readability and clear arrangement should be maintained; the legends can then be deleted.
If due to relevant data gaps, an indicator cannot be declared in a robust way, then the abbreviation “IND” (indicator not declared)
should be used for this indicator.
• 0 - calculated value is 0
• 0 - value falls under the cut-off
• 0 - assumption which exclude any flows (e.g. exported
electricity A1-A3)
• IND – in cases where the inventory does not support
the methodological approach or the calculation of the
specific indicator IND shall be used.
If no reference service life is declared (see chapter 2.13 "Reference Service Life"), the LCA results of the modules B1-B2 and B6-B7
shall refer to a period of one year. This shall then be indicated as an explanatory text below the tables. In addition, the formula for the
quantification of such B-modules over the total life cycle shall be provided.
DESCRIPTION OF THE SYSTEM BOUNDARY (X = INCLUDED IN LCA; ND = MODULE OR INDICATOR NOT DECLARED; MNR =
MODULE NOT RELEVANT)
BENEFITS
AND LOADS
CONSTRUCTION
BEYOND
PRODUCT STAGE PROCESS USE STAGE END OF LIFE STAGE
THE SYSTEM
STAGE
BOUNDARIE
S
la ire ta m w a Ry lp p u s tro p s n a rT g n iru tc a fu n a M e h t m o rf tro p s n a rTe tis e h t o t e ta g y lb m e s s A e s U e c n a n e tn ia M ria p e R tn e m e c a lp e R tn e m h s ib ru fe R y g re n e la n o ita re p Oe s u re ta w la n o ita re p Oe s u n o itc u rts n o c -e Dn o itilo m e d tro p s n a rT g n is s e c o rp e ts a W la s o p s iD -e s u e R-y re v o c e R-g n ilc y c e Rla itn e to p
A1 A2 A3 A4 A5 B1 B2 B3 B4 B5 B6 B7 C1 C2 C3 C4 D
X X X X X MND MND MNR MNR MNR MND MND X X X X X
RESULTS OF THE LCA - ENVIRONMENTAL IMPACT according to EN 15804+A2: 1 piece, Double cylinder - penta, quattro,
gemini, expert, matrix
Parameter Unit A1-A3 A4 A5 C1 C2 C3 C4 D
GWP-total kg CO 2 eq 3.89E-01 9.5E-02 4.7E-02 0 1E-03 1.6E-02 0 -1.01E-01
GWP-fossil kg CO 2 eq 4.22E-01 9.4E-02 1E-03 0 1E-03 1.6E-02 0 -1.01E-01
GWP-biogenic kg CO 2 eq -3.48E-02 9.16E-04 4.6E-02 0 4.79E-05 3.65E-07 0 2.86E-04
GWP-luluc kg CO 2 eq 6.23E-04 2.02E-06 7.76E-07 0 2.47E-08 8.85E-07 0 -1.48E-04
ODP kg CFC11 eq 3.71E-13 7.39E-18 8.5E-18 0 1.09E-19 7.9E-18 0 -3.13E-16
AP mol H+ eq 3.12E-03 3.29E-04 1.32E-05 0 1.04E-06 2.79E-06 0 -6.09E-04
EP-freshwater kg P eq 1.57E-06 1.62E-08 1.66E-09 0 2.22E-10 1.26E-09 0 -5.01E-08
EP-marine kg N eq 3.05E-04 1.44E-04 4.77E-06 0 3.3E-07 6.29E-07 0 -6.2E-05
EP-terrestrial mol N eq 3.42E-03 2E-03 5.95E-05 0 3.67E-06 1.27E-05 0 -6.66E-04
kg NMVOC
POCP 9.84E-04 4.14E-04 1.27E-05 0 9.33E-07 1.74E-06 0 -2.03E-04
eq
ADPE kg Sb eq 1.02E-04 2.69E-09 1.34E-10 0 3.11E-11 1.08E-10 0 -3.5E-06
ADPF MJ 5.56E+00 1.29E+00 1.5E-02 0 1.5E-02 7E-03 0 -1.17E+00
m3 world eq
WDP 1.41E-01 1.5E-04 6E-03 0 2.03E-06 2E-03 0 -3.3E-02
deprived
GWP = Global warming potential; ODP = Depletion potential of the stratospheric ozone layer; AP = Acidification potential of land and water; EP =
Eutrophication potential; POCP = Formation potential of tropospheric ozone photochemical oxidants; ADPE = Abiotic depletion potential for non-fossil
resources; ADPF = Abiotic depletion potential for fossil resources; WDP = Water (user) deprivation potential)
RESULTS OF THE LCA - INDICATORS TO DESCRIBE RESOURCE USE according to EN 15804+A2: 1 piece, Double cylinder -
penta, quattro, gemini, expert, matrix
Parameter Unit A1-A3 A4 A5 C1 C2 C3 C4 D
PERE MJ 4.36E+00 3E-03 4.02E-01 0 4.63E-05 2E-03 0 -1.73E-01
PERM MJ 3.99E-01 0 -3.99E-01 0 0 0 0 0
PERT MJ 4.76E+00 3E-03 3E-03 0 4.63E-05 2E-03 0 -1.73E-01
PENRE MJ 5.47E+00 1.29E+00 1.5E-02 0 1.5E-02 1.05E-01 0 -1.18E+00
5 Environmental-Product Declaration - dormakaba - Reversible Double Cylinder - penta, quattro, gemini, expert, matrix
PENRM MJ 9.8E-02 0 0 0 0 -9.8E-02 0 0
PENRT MJ 5.56E+00 1.29E+00 1.5E-02 0 1.5E-02 7E-03 0 -1.18E+00
SM kg 2.28E-01 0 0 0 0 0 0 0
RSF MJ 0 0 0 0 0 0 0 0
NRSF MJ 0 0 0 0 0 0 0 0
FW m3 3.8E-03 6.25E-06 1.38E-04 0 8.31E-08 3.83E-05 0 -1E-03
PERE = Use of renewable primary energy excluding renewable primary energy resources used as raw materials; PERM = Use of renewable primary
energy resources used as raw materials; PERT = Total use of renewable primary energy resources; PENRE = Use of non-renewable primary energy
excluding non-renewable primary energy resources used as raw materials; PENRM = Use of non-renewable primary energy resources used as raw
materials; PENRT = Total use of non-renewable primary energy resources; SM = Use of secondary material; RSF = Use of renewable secondary fuels;
NRSF = Use of non-renewable secondary fuels; FW = Use of net fresh water
RESULTS OF THE LCA – WASTE CATEGORIES AND OUTPUT FLOWS according to EN 15804+A2:
1 piece, Double cylinder - penta, quattro, gemini, expert, matrix
Parameter Unit A1-A3 A4 A5 C1 C2 C3 C4 D
HWD kg 2.63E-08 1.23E-10 2.2E-11 0 1.43E-12 2.77E-11 0 -4.84E-09
NHWD kg 7E-02 1.3E-04 1E-03 0 1.5E-06 2E-03 0 -1.5E-02
RWD kg 2.7E-04 1.12E-06 7.83E-07 0 1.58E-08 2.69E-07 0 -2.05E-05
CRU kg 0 0 0 0 0 0 0 0
MFR kg 0 0 0 0 0 2.17E-01 0 0
MER kg 0 0 0 0 0 0 0 0
EEE MJ 2.6E-02 0 7.1E-02 0 0 0 0 0
EET MJ 4.7E-02 0 1.29E-01 0 0 0 0 0
HWD = Hazardous waste disposed; NHWD = Non-hazardous waste disposed; RWD = Radioactive waste disposed; CRU = Components for re-use;
MFR = Materials for recycling; MER = Materials for energy recovery; EEE = Exported electrical energy; EET = Exported thermal energy
RESULTS OF THE LCA – additional impact categories according to EN 15804+A2-optional:
1 piece, Double cylinder - penta, quattro, gemini, expert, matrix
Parameter Unit A1-A3 A4 A5 C1 C2 C3 C4 D
Disease
PM 1.4E-02 0 0 ND ND 0 0 0
incidence
IR kBq U235 eq 0 0 0 ND ND 0 0 0
ETP-fw CTUe 0 0 0 ND ND 0 0 0
HTP-c CTUh 0 0 0 ND ND 0 0 0
HTP-nc CTUh 0 0 0 ND ND 0 0 0
SQP SQP 0 0 0 ND ND 0 0 0
PM = Potential incidence of disease due to PM emissions; IR = Potential Human exposure efficiency relative to U235; ETP-fw = Potential comparative
Toxic Unit for ecosystems; HTP-c = Potential comparative Toxic Unit for humans (cancerogenic); HTP-nc = Potential comparative Toxic Unit for humans
(not cancerogenic); SQP = Potential soil quality index
Disclaimer 1 – for the indicator “Potential Human exposure efficiency relative to U235”. This impact category deals mainly with the
eventual impact of low dose ionizing radiation on human health of the nuclear fuel cycle. It does not consider effects due to possible
nuclear accidents, occupational exposure nor due to radioactive waste disposal in underground facilities. Potential ionizing radiation
from the soil, from radon and from some construction materials is also not measured by this indicator.
Disclaimer 2 – for the indicators “abiotic depletion potential for non-fossil resources”, “abiotic depletion potential for fossil resources”,
“water (user) deprivation potential, deprivation-weighted water consumption”, “potential comparative toxic unit for ecosystems”,
“potential comparative toxic unit for humans – cancerogenic”, “Potential comparative toxic unit for humans - not cancerogenic”,
“potential soil quality index”. The results of this environmental impact indicator shall be used with care as the uncertainties on these
results are high or as there is limited experienced with the indicator.
References
DIN 18252 DIN EN ISO 14025
DIN 18252: 2018, Profile cylinders for door locks – Terminology, DIN EN ISO 14025:2011, Environmental labels and
dimensions, requirements, test methods and marking declarations - Type III environmental declarations - Principles
and procedures.
DIN EN 1303
DIN EN 1303: EN 15804
2015, Building Hardware - Cylinders for locks - Requirements EN 15804:2019+A2, Sustainability of
and test methods construction works — Environmental Product
Declarations — Core rules for the product category of
DIN EN 1634-1 construction products.
DIN EN 1634-1:2018, Fire resistance and smoke control tests
for door and shutter assemblies, openable windows and REACH Regulation
elements of building hardware REACH Regulation (EC) No 1907/2006 of the European
Parliament and of the Council on the Registration,
DIN EN 1634-2 Evaluation, Authorisation and Restriction of Chemicals.
DIN EN 1634-2:2009, Fire resistance and smoke control tests
for door, shutter and openable window assemblies and RoHS 2011/65/EU
elements of building hardware RoHS 2011/65/EU, Directive on the restriction of the use of
certain
6 Environmental-Product Declaration - dormakaba - Reversible Double Cylinder - penta, quattro, gemini, expert, matrix
hazardous substances in electrical and electronic equipment. (https://www.gabi-software.com/support/gabi/gabidatabase-
2020-lci-documentation/).
European Chemicals Agency (ECHA)
https://echa.europa.eu/de/ LCA-tool dormakaba
LCA tool, version 1.0.
Further References Developed by Sphera Solutions GmbH
IBU PCR Part A
Institut Bauen PCR – Part A: Calculation Rules for the Life Cycle Assessment
und Umwelt e.V.: General Instructions for the EPD Programme and Requirements on the Project Re-port
of according to EN 15804+A2:2019, Version 1.0, Institut
Institut Bauen und Umwelt e.V. Version 2.0., Berlin: Institut Bauen und Umwelt e.V., www.ibu-epd.com.
Bauen
und Umwelt e.V., 2021. www.ibu-epd.com
PCR Part B
GaBi ts software PCR – Part B: Requirements on the EPD for Electronic and
Sphera Solutions GmbH physical Access Control Systems , version 1.2, Institut Bauen
Gabi Software System and Database for Life Cycle und
Engineering 1992-2020 Umwelt e.V., www.ibu-epd.com, 2017.
Version 10.0.0.71 The literature referred to in the Environmental Product
University of Stuttgart, Leinfelden-Echterdingen Declaration must be listed in full.Standards already fully quoted
in the EPD do not need to be listed here again.
GaBi ts documentation The current version of PCR Part A and PCR Part B of the PCR
GaBi life cycle inventory data documentation document on which they are based must be referenced.
7 Environmental-Product Declaration - dormakaba - Reversible Double Cylinder - penta, quattro, gemini, expert, matrix
Publisher
Institut Bauen und Umwelt e.V. +49 (0)30 3087748- 0
Hegelplatz 1 info@ibu-epd.com
10117 Berlin www.ibu-epd.com
Germany
Programme holder
Institut Bauen und Umwelt e.V. +49 (0)30 3087748- 0
Hegelplatz 1 info@ibu-epd.com
10117 Berlin www.ibu-epd.com
Germany
Author of the Life Cycle Assessment
Sphera Solutions GmbH +49 711 341817-0
Hauptstraße 111- 113 info@sphera.com
70771 Leinfelden-Echterdingen www.sphera.com
Germany
Owner of the Declaration
dormakaba International Holding GmbH +49 2333 793-0
DORMA Platz 1 info.de@dormakaba.com
58256 Ennepetal www.dormakaba.com
Germany
8 Environmental-Product Declaration - dormakaba - Reversible Double Cylinder - penta, quattro, gemini, expert, matrix
