ENVIRONMENTAL PRODUCT DECLARATION
as per ISO 14025 and EN 15804+A2
Owner of the Declaration Branth-Chemie A.V. Branth KG
Publisher Institut Bauen und Umwelt e.V. (IBU)
Programme holder Institut Bauen und Umwelt e.V. (IBU)
Declaration number EPD-BRC-20240259-CBC1-EN
Issue date 22.11.2024
Valid to 21.11.2029
Brantho-Korrux/Powercoat 3 in 1
Branth-Chemie A.V.Branth KG
www.ibu-epd.com | https://epd-online.com
General Information
Branth-Chemie A.V.Branth KG Brantho-Korrux/Powercoat 3 in 1
Programme holder Owner of the declaration
IBU – Institut Bauen und Umwelt e.V. Branth-Chemie A.V. Branth KG
Hegelplatz 1 Biedenkamp 23
10117 Berlin 21509 Glinde
Germany Germany
Declaration number Declared product / declared unit
EPD-BRC-20240259-CBC1-EN 1 kg of Brantho-Korrux 3 in 1 / Powercoat 3 in 1
This declaration is based on the product category rules: Scope:
Coatings with organic binders, 01.08.2021 The EPD is applicable for the Brantho-Korrux 3 in 1/ Power Coat 3 in 1
(PCR checked and approved by the SVR) products.
The products are produced at the Branth production site in Glinde near
Issue date Hamburg in Germany. The declaration is for the environmental impact of
an average product composition (average EPD).
22.11.2024
The owner of the declaration shall be liable for the underlying information
and evidence; the IBU shall not be liable with respect to manufacturer
Valid to
information, life cycle assessment data and evidences.
21.11.2029
The EPD was created according to the specifications of EN 15804+A2. In
the following, the standard will be simplified as EN 15804.
Verification
The standard EN 15804 serves as the core PCR
Independent verification of the declaration and data according to ISO
14025:2011
internally X externally
Dipl.-Ing. Hans Peters
(Chairman of Institut Bauen und Umwelt e.V.)
Florian Pronold Ms Jane Anderson,
(Managing Director Institut Bauen und Umwelt e.V.) (Independent verifier)
1 Environmental Product Declaration - Branth-Chemie A.V.Branth KG - Brantho-Korrux/Powercoat 3 in 1
Product
Name Value Unit
Product description/Product definition
1100 -
Brantho-Korrux 3 in 1 / Power Coat 3 in 1 is a one-component Density kg/m3
1500
solvent based (aromatic-free) paint for corrosion protection of
Density 1.1-1.5 kg/ltr.
constructions, buildings, machines and transport vehicles in
rural-, urban-, industrial- and maritime areas. Brantho-Korrux 3 Solids content 69 - 73 %
in 1 / Power Coat 3 in 1 has a semi gloss finish (except effect Gloss (Lacke) 40 - 70 %
colours). Viscosity 155 - 175 s; DIN 4mm
For the use and application of the product the respective
Corrosion level C1, C2,
national provisions at the place of use apply.
(DIN EN ISO C3, C4, Corrosion Category
12944) C5, CX
Application
Brantho-Korrux 3 in 1 / Power Coat 3 in 1 can be applied using NORSOK 300 µm DFT
a roller, brush or by spray application techniques. Dipping is standards
also possible. primer, pigmented, solvent
Ist is suitable for all metal surfaces, concrete, most hard GISBAU M-GP02 based, free of aromatic
pastics, glas, screed, old coatings, rust, etc. hydrocarbons
The product is suitable: coating, solvent based,
GISBAU M-LL01
• as a protective coating for new construction or aromatic free
maintenance DIN 4102-1 (on
A1/A2 not-flammable
• as both primer and topcoat metals)
• as a primer for 1-component and most 2-component Indoor Air
A+ -
finishes Pollution
• for constructions built from several types of materials
Approved for steel-
DIN 55928-5 Ü-mark
• as a substitute for toxic red-lead primer (tested by the constructions and equipment
German Railway authorities) One-Component-special
Decopaint-
• as a substitute for environmentally unfriendly PVC / Chl. II1i coating, Metal-high-build
directives
Rubber coatings coating (bulding)
• as a substitute for epoxy coatings (partly)
One-component-coating,
• as a substitute for simple and complicated alkyd Decopaint-
II2e underbody protection coating
coatings directives
(vehicle repair)
This product is not recommended for application on soft plastics Product for which no legal provisions for harmonisation of the
or exterior application on wood, as it is not vapour permeable. EU exist.
Baking or forced curing (heat) is NOT POSSIBLE. For the use and application of the product the respective
The substrate should be dry, solid and free of contaminants. national provisions at the place of use apply, in Germany for
Stir well before application (by hand or machine). example the building codes of the federal states and the
Possible application and drying temperature from minus 10° C corresponding national specifications.
to plus 30° C.
Base materials/Ancillary materials
Ideal application and drying temperature from plus 15° C to plus
Brantho-Korrux 3 in 1 / Power Coat 3 in 1 comprise the
25o C.
following substances:
Product for which no legal provisions for harmonisation of the Name Value Unit
EU exist. Binders 20-40 %
For the use and application of the product the respective
Organic pigments 0.5-2 %
national provisions at the place of use apply, in Germany for
Inorganic fillers/pigments 25-50 %
example the building codes of the federal states and the
additives 15-35 %
corresponding national specifications.
This product/article/at least one partial article contains
Technical Data
substances listed in the candidate list of substances of very
A CE-marking does not exists for coatings as they are semi- high concern (SVHC) for authorisation (date: 27.06.2018)
finished products whose final state is achieved by its proper exceeding 0.1 percentage by mass: NO
processing.
Therefore properties in liquid state are listed in the following This product/article/at least one partial article contains other
chapter "Constructional data". Carcinogenic, mutagenic, reprotoxic (CMR)substances in
Constructional data categories 1A or 1B which are not on the candidate list,
exceeding 0.1 percentage by mass: NO
Biocide products were added to this construction product or it
has been treated with biocide products: NO
Biocidal Products Regulation (BPR, Regulation (EU) 528/2012)
Reference service life
The RSL is dependent on the application scenario which has
not been defined in this EPD. Paint in its original form is a semi-
2 Environmental Product Declaration - Branth-Chemie A.V.Branth KG - Brantho-Korrux/Powercoat 3 in 1
finished product. Therefore, no RSL is declared. Further found in the technical data sheet.
information about resistances (after proper processing) can be
LCA: Calculation rules
The treatment and potential benefits for avoided primary
Declared Unit production (for the net scrap amount only) are declared in
The declared unit for calculation is 1 kg of Brantho-Korrux 3 in 1 module D. The solvent emissions to air when the paint is
/ Power Coat 3 paint ready to be applied excluding packaging. applied are also declared in this module.
It is packaged in a tin can (0.097 kg).
Declared unit and mass reference End-of-Life (EoL) stage - Modules C1-C4
Name Value Unit • EoL module C1: Manual dismantling/ deconstruction
(without environmental burdens).
Declared unit 1 kg
• EoL module C2: Truck transport to waste treatment with
Gross density (mean value) 1.4 kg/ltr.
a distance of 530 km (can be adapted on building level,
Gross density (mean value) 1400 kg/m3 if relevant)
Dry layer thickness 60 µm • EoL module C4: considers disposal emissions only
Productiveness 6,4 m²/kg without benefits (100% scenario). The disposal scenario
(EU region) assumes that the coating is on a e.g., metal
This EPD declares an average composition for all products
surface during disposal and is thermally disposed off
under study. As an estimate of the robustness of the LCA
when the metal is recycled (melting). No benefits are
values, the weighted average composition of the declared
considered. Only the resulting emissions are taken into
Brantho-Korrux 3 in 1 / Powercoat 3 in 1 product is calculated
account. Module C3 is declared as 0.
relative to the production volume shares of a total of 19 variants
in scope produced at the Branth production site located in
Reuse, recovery or recycling potential beyond system
Glinde, Germany. The production process remains the same for
boundary - Module D
all variants in scope. The weighted average is representative of
Loads and benefits beyond the system boundary would be
the environemntal impacts of the 19 variants covered in scope.
declared in this module, if relevant.
System boundary
The type of EPD according to EN15804 is cradle to gate with
options, modules C1–C4, and module D. Geographic Representativeness
The following modules are declared: A1–A3, C, D and
Land or region, in which the declared product system is
additional module A5.
manufactured, used or handled at the end of the product´s
lifespan: Germany
Production stage - Modules A1-A3
The product stage includes:
Comparability
• Raw material supply (A1)
• Transport to the manufacturer (A2) Basically, a comparison or an evaluation of EPD data is only
• Manufacturing (A3), including provision of energy. possible if all the data sets to be compared were created
Packaging is also considered in this module. according to EN 15804 and the building context, respectively
the product-specific characteristics of performance, are taken
Construction stage - Module A5 into account. Background dataset : Sphera LCA FE (GaBi ts)
The construction stage considers packaging treatment software, CUP 2023.1
(recycling) of metal paint cans.
LCA: Scenarios and additional technical information
3 in 1 / Powercoat 3 in 1.
Characteristic product properties of biogenic carbon
The calculation of the biogenic carbon content in the declared
Installation into the building (A5)
product is based on the assumption of the biogenic carbon
content in the materials composition (based on the mapped Name Value Unit
Sphera LCA FE dataset). Tin packaging sent to recycling 0.097 kg
No biogenic carbon content exists in the packaging material. Solvent emissions to air (during application) 0.266 kg
Information on describing the biogenic carbon content at .
factory gate
End of life (C1-C4)
Name Value Unit
Module C1: Manual dismantling (no environmental loads).
Biogenic carbon content in product 0.0339 kg Module C2: An average transport distance of 530 km is
C assumed by truck.
Biogenic carbon content in accompanying kg Module C4: Considers disposal emissions only without benefits.
-
packaging C The disposal scenario (EU region) assumes that the coating is
on a e.g., metal surface during disposal and is thermally
Note: 1 kg of biogenic carbon is equivalent to 44/12 kg of CO .
2 disposed off when the metal is recycled (melting/incineration).
No benefits are awarded for incineration due to energy
substitution, but only the resulting emissions are taken into
The following technical scenario information is used to calculate
account. A conservative approach of End of Life with cut off is
the declared modules.
considered, so no energy benefits are applied.
The values refer to the declared unit of 1 kg of Brantho-Korrux
3 Environmental Product Declaration - Branth-Chemie A.V.Branth KG - Brantho-Korrux/Powercoat 3 in 1
Name Value Unit scenario information
Thermal utilization without energy recovery 0.734 kg
This module considers the benefits of packaging treatment
(metal recycling) only
Reuse, recovery and/or recycling potentials (D), relevant
4 Environmental Product Declaration - Branth-Chemie A.V.Branth KG - Brantho-Korrux/Powercoat 3 in 1
LCA: Results
The following tables display the environmentally relevant results according to EN 15804 for 1 kg of Brantho-Korrux 3 in 1 / Powercoat 3
in 1.
DESCRIPTION OF THE SYSTEM BOUNDARY (X = INCLUDED IN LCA; MND = MODULE OR INDICATOR NOT DECLARED; MNR
= MODULE NOT RELEVANT)
Benefits and
Construction loads beyond
Product stage Use stage End of life stage
process stage the system
boundaries
la ire ta m w a Ry lp p u s tro p s n a rT g n iru tc a fu n a M e h t m o rf tro p s n a rTe tis e h t o t e ta g y lb m e s s A e s U e c n a n e tn ia M ria p e R tn e m e c a lp e R tn e m h s ib ru fe R y g re n e la n o ita re p Oe s u re ta w la n o ita re p Oe s u n o itc u rts n o c -e Dn o itilo m e d tro p s n a rT g n is s e c o rp e ts a W la s o p s iD -e s u e R-y re v o c e R-g n ilc y c e Rla itn e to p
A1 A2 A3 A4 A5 B1 B2 B3 B4 B5 B6 B7 C1 C2 C3 C4 D
X X X MND X MND MND MNR MNR MNR MND MND X X X X X
RESULTS OF THE LCA - ENVIRONMENTAL IMPACT according to EN 15804+A2: 1 kg Brantho-Korrux/Powercoat 3 in 1
Parameter Unit A1-A3 A5 C1 C2 C3 C4 D
GWP-total kg CO 2 eq 1.95E+00 1.39E-01 0 2.89E-02 0 1.98E+00 -1.32E-01
GWP-fossil kg CO 2 eq 2.33E+00 1.39E-01 0 2.85E-02 0 1.86E+00 -1.32E-01
GWP-biogenic kg CO 2 eq -3.81E-01 0 0 8.43E-05 0 1.25E-01 6.72E-05
GWP-luluc kg CO 2 eq 8.63E-04 0 0 2.64E-04 0 3.97E-05 -2.72E-06
ODP kg CFC11 eq 7.32E-12 0 0 3.71E-15 0 6.29E-13 -2.88E-16
AP mol H+ eq 7.02E-03 0 0 2.82E-05 0 3.13E-04 -2.83E-04
EP-freshwater kg P eq 1.15E-05 0 0 1.04E-07 0 1.59E-07 -2.39E-08
EP-marine kg N eq 1.48E-03 0 0 8.02E-06 0 6.99E-05 -4.97E-05
EP-terrestrial mol N eq 1.6E-02 0 0 1.01E-04 0 1.46E-03 -4.37E-04
kg NMVOC
POCP 1.01E-02 1.29E-01 0 2.35E-05 0 1.93E-04 -2.02E-04
eq
ADPE kg Sb eq 9.96E-06 0 0 1.88E-09 0 4.93E-09 -3.28E-07
ADPF MJ 4.78E+01 0 0 3.89E-01 0 9.42E-01 -1.21E+00
m3 world eq
WDP 4.88E-01 0 0 3.45E-04 0 1.73E-01 -2.45E-02
deprived
GWP = Global warming potential; ODP = Depletion potential of the stratospheric ozone layer; AP = Acidification potential of land and water; EP =
Eutrophication potential; POCP = Formation potential of tropospheric ozone photochemical oxidants; ADPE = Abiotic depletion potential for non-fossil
resources; ADPF = Abiotic depletion potential for fossil resources; WDP = Water (user) deprivation potential)
RESULTS OF THE LCA - INDICATORS TO DESCRIBE RESOURCE USE according to EN 15804+A2: 1 kg Brantho-
Korrux/Powercoat 3 in 1
Parameter Unit A1-A3 A5 C1 C2 C3 C4 D
PERE MJ 2.98E+00 0 0 2.83E-02 0 2.29E+00 7.62E-02
PERM MJ 1.98E+00 0 0 0 0 -1.98E+00 0
PERT MJ 4.96E+00 0 0 2.83E-02 0 3.1E-01 7.62E-02
PENRE MJ 1.98E+01 0 0 3.9E-01 0 2.9E+01 -1.21E+00
PENRM MJ 2.8E+01 0 0 0 0 -2.8E+01 0
PENRT MJ 4.79E+01 0 0 3.9E-01 0 9.43E-01 -1.21E+00
SM kg 2.1E-02 0 0 0 0 0 7.6E-02
RSF MJ 0 0 0 0 0 0 0
NRSF MJ 0 0 0 0 0 0 0
FW m3 1.72E-02 0 0 3.1E-05 0 4.16E-03 -5.53E-04
PERE = Use of renewable primary energy excluding renewable primary energy resources used as raw materials; PERM = Use of renewable primary
energy resources used as raw materials; PERT = Total use of renewable primary energy resources; PENRE = Use of non-renewable primary energy
excluding non-renewable primary energy resources used as raw materials; PENRM = Use of non-renewable primary energy resources used as raw
materials; PENRT = Total use of non-renewable primary energy resources; SM = Use of secondary material; RSF = Use of renewable secondary fuels;
NRSF = Use of non-renewable secondary fuels; FW = Use of net fresh water
RESULTS OF THE LCA – WASTE CATEGORIES AND OUTPUT FLOWS according to EN 15804+A2:
1 kg Brantho-Korrux/Powercoat 3 in 1
Parameter Unit A1-A3 A5 C1 C2 C3 C4 D
HWD kg 3.83E-09 0 0 1.21E-12 0 3.25E-14 -9.34E-12
NHWD kg 8.17E-01 0 0 5.95E-05 0 1.85E-01 1.83E-02
RWD kg 8.55E-04 0 0 7.3E-07 0 3.17E-05 1.5E-07
CRU kg 0 0 0 0 0 0 0
MFR kg 0 9.7E-02 0 0 0 0 0
MER kg 0 0 0 0 0 0 0
EEE MJ 0 0 0 0 0 0 0
5 Environmental Product Declaration - Branth-Chemie A.V.Branth KG - Brantho-Korrux/Powercoat 3 in 1
EET MJ 0 0 0 0 0 0 0
HWD = Hazardous waste disposed; NHWD = Non-hazardous waste disposed; RWD = Radioactive waste disposed; CRU = Components for re-use;
MFR = Materials for recycling; MER = Materials for energy recovery; EEE = Exported electrical energy; EET = Exported thermal energy
RESULTS OF THE LCA – additional impact categories according to EN 15804+A2-optional:
1 kg Brantho-Korrux/Powercoat 3 in 1
Parameter Unit A1-A3 A5 C1 C2 C3 C4 D
Disease
PM 6.62E-08 0 0 2.14E-10 0 3.58E-09 -4E-09
incidence
IR kBq U235 eq 9.77E-02 0 0 1.09E-04 0 3.35E-03 2.96E-03
ETP-fw CTUe 2.6E+01 3.21E-01 0 2.76E-01 0 3.04E-01 -7.45E-02
HTP-c CTUh 1.08E-09 0 0 5.65E-12 0 2.89E-11 -5.38E-11
HTP-nc CTUh 7.38E-08 1.97E-09 0 2.97E-10 0 2.54E-09 -1.78E-09
SQP SQP 8.85E+00 0 0 1.62E-01 0 2.8E-01 1.46E-02
PM = Potential incidence of disease due to PM emissions; IR = Potential Human exposure efficiency relative to U235; ETP-fw = Potential comparative
Toxic Unit for ecosystems; HTP-c = Potential comparative Toxic Unit for humans (cancerogenic); HTP-nc = Potential comparative Toxic Unit for humans
(not cancerogenic); SQP = Potential soil quality index
Disclaimer 1 – for the indicator “Potential Human exposure efficiency relative to U235”. This impact category deals mainly with the
eventual impact of low-dose ionizing radiation on human health of the nuclear fuel cycle. It does not consider effects due to possible
nuclear accidents, occupational exposure or radioactive waste disposal in underground facilities. Potential ionizing radiation from the
soil, radon and from some construction materials is also not measured by this indicator.
Disclaimer 2 – for the indicators “abiotic depletion potential for non-fossil resources”, “abiotic depletion potential for fossil resources”,
“water (user) deprivation potential, deprivation-weighted water consumption”, “potential comparative toxic unit for ecosystems”,
“potential comparative toxic unit for humans – cancerogenic”, “Potential comparative toxic unit for humans - not cancerogenic”,
“potential soil quality index”. The results of this environmental impact indicator shall be used with care as the uncertainties on these
results are high as there is limited experience with the indicator.
References
Standards 528/2012)
Regulation (EU) No 528/2012 of the European Parliament and
DIN EN ISO 12944 of the Council of 22 May 2012 concerning the making available
Paints and varnishes - Corrosion protection of steel structures on the market and use of biocidal products
by protective paint systems
Decopaint-directives
DIN EN ISO 14001 Limitation of emissions / /EU Directive 2004/2
Environmental management systems - Requirements with
guidance for use (ISO 14001:2015); German and English EMAS
version EN ISO 14001:2015 Eco-Management and Audit Scheme: www.emas.de
DIN EN ISO 14025 Emissions Dans L'Air Interieur / Indoor air pollution
EN ISO 14025:2011, Environmental labels and declarations — classification
Type III environmental declarations — Principles and VOC Regulation for construction products and furnishing and
procedures. equipment materials: https://www.eco-
institut.de/de/portfolio/emissions-dans-lair-interieur/
DIN EN 15804
EN 15804:2012+A2:2019+AC:2021, Sustainability of GISBAU
construction works — Environmental Product Declarations — Gefahrstoff-Informationssystem der BG BAU (Hazardous
Core rules for the product category of construction products. substance information system of the BG BAU):
www.bgbau.de/themen/sicherheit-und-
DIN 4102-1 gesundheit/gefahrstoffe/gisbau
Fire behaviour of building materials and building components -
Part 1: Building materials; concepts, requirements and tests NORSOK standards
1998 www.standard.no/en/sectors/petroleum/norsok-standards/
DIN 55928-5 P221159697 MPA - NRW REACH
Binders for paints and varnishes - Refined soya bean oil - Regulation (EC) No 1907/2006 of the European Parliament and
Requirements and methods of test: Approval for steel- of the Council of 18th December 2006 concerning the
constructions and -equipment (Ü-mark) Registration, Evaluation, Authorisation and Restriction of
Chemicals (REACH)
DIN EN 71-3
Safety of toys - Part 3: Migration of certain elements; German ROHS 2011/65/EURegulation (EC) No 65/2011 and No
version EN 71-3:2019+A1:2021 863/2015 of the European Parliament and of the Council of 8th
june 2011 and 31st march 2015 concerning the restriction of the
DIN EN ISO 9001 use of certain hazardous substances in electrical and electronic
Quality management systems - Requirements (ISO 9001:2015); equipment
German and English version EN ISO 9001:2015
Biocidal Products Regulation (BPR, Regulation (EU)
6 Environmental Product Declaration - Branth-Chemie A.V.Branth KG - Brantho-Korrux/Powercoat 3 in 1
Further References PCR Part B
PCR – Part B: Requirements of the EPD for Coatings with
IBU 2021 organic binders, v5, Institut Bauen und Umwelt e.V., www.bau-
Institut Bauen und Umwelt e.V.: General Instructions for the umwelt.com, 2023
EPD programme of Institut Bauen und Umwelt e.V., Version
2.0, Berlin: Institut Bauen und Umwelt e.V., 2021 Sphera LCA FE (GaBi ts)
www.ibu-epd.com GaBi ts dataset documentation for the software-system and
databases, LBP, University of Stuttgart and
PCR Part A thinkstep,Leinfelden-Echterdingen, 2023
PCR - Part A: Calculation rules for the Life Cycle Assessment (https://www.gabisoftware.com/support/gabi).
and Requirements on the BackgroundReport, version 1.3,
Institut Bauen und Umwelt e.V., 2021. .
7 Environmental Product Declaration - Branth-Chemie A.V.Branth KG - Brantho-Korrux/Powercoat 3 in 1
Publisher
Institut Bauen und Umwelt e.V. +49 (0)30 3087748- 0
Hegelplatz 1 info@ibu-epd.com
10117 Berlin www.ibu-epd.com
Germany
Programme holder
Institut Bauen und Umwelt e.V. +49 (0)30 3087748- 0
Hegelplatz 1 info@ibu-epd.com
10117 Berlin www.ibu-epd.com
Germany
Author of the Life Cycle Assessment
Sphera Solutions GmbH +49 711 341817-0
Hauptstraße 111- 113 info@sphera.com
70771 Leinfelden-Echterdingen www.sphera.com
Germany
Owner of the Declaration
Branth-Chemie A.V. Branth KG +494036974020
Biedenkamp 23 postmaster@branth-chemie.de
21509 Glinde www.branth-chemie.de
Germany
8 Environmental Product Declaration - Branth-Chemie A.V.Branth KG - Brantho-Korrux/Powercoat 3 in 1
