ENVIRONMENTAL PRODUCT DECLARATION
as per ISO 14025 and EN 15804+A2
Owner of the Declaration Vitrulan Textile Glass GmbH
Publisher Institut Bauen und Umwelt e.V. (IBU)
Programme holder Institut Bauen und Umwelt e.V. (IBU)
Declaration number EPD-VIT-20230430-CBC1-EN
Issue date 09.01.2024
Valid to 08.01.2029
Woven glass fibre wall covering
Vitrulan Textile Glass GmbH
www.ibu-epd.com | https://epd-online.com
General Information
Vitrulan Textile Glass GmbH Woven glass fibre wall covering
Programme holder Owner of the declaration
IBU – Institut Bauen und Umwelt e.V. Vitrulan Textile Glass GmbH
Hegelplatz 1 Bernecker Straße 8
10117 Berlin 95509 Marktschorgast
Germany Germany
Declaration number Declared product / declared unit
EPD-VIT-20230430-CBC1-EN 1 m2 of woven glass fibre wall covering with an average grammage of
around 0.145 kg/m2.
This declaration is based on the product category rules: Scope:
Wall coverings, 01.08.2021 This specific EPD document refers to woven glass fibre wall covering
(PCR checked and approved by the SVR) produced by Vitrulan Textile Glass GmbH. The production data was
recorded in 2021. The production plant is located in Marktschorgast,
Germany.
Issue date
The owner of the declaration shall be liable for the underlying information
09.01.2024
and evidence; the IBU shall not be liable with respect to manufacturer
information, life cycle assessment data and evidences.
Valid to
The EPD was created according to the specifications of EN 15804+A2. In
08.01.2029 the following, the standard will be simplified as EN 15804.
Verification
The standard EN 15804 serves as the core PCR
Independent verification of the declaration and data according to ISO
14025:2011
internally X externally
Dipl.-Ing. Hans Peters
(Chairman of Institut Bauen und Umwelt e.V.)
Florian Pronold Vito D'Incognito,
(Managing Director Institut Bauen und Umwelt e.V.) (Independent verifier)
1 Environmental Product Declaration - Vitrulan Textile Glass GmbH - Woven glass fibre wall covering
Product
3. AVOIDING TEXTURAL DIFFERENCES: Never paste
Product description/Product definition the wall covering upside down or inside out. Some
Woven glass fibre wall covering, manufactured by Vitrulan products have a handy mark on the back of the wall
Textile Glass GmbH, is made of glass yarns and used for both, covering which serves as a guide. These marks are
functional and decorative purposes. It is generally distinguished spaced at approximately 1 m intervals from one length
from wall paperings based on a paper substrate by a high- to the next. Butt-joining: Make sure that the edges butt
quality special glass woven fabric which is used as the up smoothly where one length joins another. Important:
substrate material. The glass fibre wall covering is a structured, Make sure that the thread path in the weave of each
patterned or practically smooth fabric comprising glass yarns subsequent length lines up with the previous one at eye
arranged vertically and horizontally. Generally, it is glued on level. With straight match: We weave an alignment
walls and ceilings and painted afterwards. It may include white guide into wallcoverings with large-format repeated
pigments to reduce processing time on the construction site. It patterns to make it easier to align them: a yellow thread
is particularly easy to handle: it does not shrink or stretch, is which is visible on both sides of the covering. When
easy to cut and produces perfect seams. It reinforces walls, applying each consecutive length, simply make sure
covers cracks, and prevents new cracks from forming. that the yellow thread is perfectly aligned with the yellow
thread in the previous length.
During application, the wall or ceiling is pasted and then the 4. PRESSING ON AND TRIMMING: Use a (hard plastic)
strip of wall covering is hung on the prepared paste bed, or, wallpaper spatula and press down firmly across the
alternatively, the wall covering comes with a water-activatable entire length, smoothing out any air bubbles. Carefully
adhesive which is already applied to the wall covering's backing press (the) overlapping fabric into the corners and cut
– this adhesive can be easily activated by water using the with a sharp knife.
'Aqua-Quick device' specially developed for this purpose. 5. PAINTING: Apply the paint evenly, once the wall
Vitrulan's Aqua Technology facilitates work and reduces covering has completely dried. Follow the paint
processing times for the user. manufacturer's instructions. The need for further
coatings depends on the paint quality, degree of gloss,
Since woven glass fibre wall coverings are designed to shade, expected stress, lighting situation and desired
reinforce walls and ceilings, they are bonded to the building's surface appearance. With raised fibres: Slight sanding
structure. This means that they are disposed of as construction between coatings is possible.
waste. Waste arising from installation can generally be
disposed of as household waste since glass fibre wall Technical Data
coverings are not classed as special waste. Our woven glass Main characteristics of our woven glass fibre wall covering are:
fibre wall covering is OEKO-TEX-certified and completely non-
• Superb reaction to fire: B-s1, d0 according to DIN EN
hazardous to health. Sustainable interior design and premium
13501-1
product quality are hallmarks of all our textile glass fibre wall
• Wall reinforcing and crack bridging
coverings.
• Impact and perforation resistant
• Abrasion and scrub resistant (depending on the coating)
For the placing on the market of the product in the European
• Resistant to disinfectants and cleaning agents
Union/European Free Trade Association (EU/EFTA) (with the
(depending on the coating)
exception of Switzerland) Regulation (EU) No. 305/2011 (CPR)
• Non-toxic and food-safe: OEKO-TEX-certified
applies. The product needs a declaration of performance taking
• Water vapour permeable
into consideration EN 15102:2007+A1:2011 and the CE-
• Suitable for allergy sufferers
marking. For application and use, the respective national
• In addition to the many technical benefits, our woven
provisions apply.
glass fibre wall coverings provide almost limitless scope
for creativity when it comes to interior design
Application
Woven glass fibre wall coverings are used indoors on ceilings
and walls in the following steps. More details are to be found in Constructional data
the technical data sheets. Name Value Unit
1. PREPARATION: Substrates should be dry, clean, B-s1,
Fire behaviour according to DIN EN 13501-1 -
smooth and stable. Pretreat absorbent substrates with a d0
suitable primer. Do not apply with room and surface Release of formaldehyde max. < 120 mg/kg
passed -
temperatures below +8 °C. Use the same serial according to DIN EN 12149
numbers when applying to adjacent areas. One drop =
Migration of heavy metals (max.) and certain
wall height plus 5–10 cm. passed -
other elements to DIN EN 12149
2. APPLYING ADHESIVE: (a) Without Aqua Technology,
Vinyl chloride monomer (VCM) content max.
apply sufficient latex adhesive with a paint roller or passed -
< 0,2 mg/kg according to DIN EN 12149
airless spray gun evenly to the wall over a width of 1–2
sheets. Observe the adhesive manufacturer's Sound absorption according to EN ISO 354, EN NPD -
application notes. This also applies for applications with ISO 11654
a wall-papering device. (b) With Aqua Technology the Thermal resistance according to EN 12667, EN
NPD -
wall covering comes with a water-activatable adhesive 12524
which is already applied to the wall covering's backing.
This adhesive can be easily activated by water using the
Performance data of the product in accordance with the
'Aqua-Quick device'. At normal room
declaration of performance with respect to its essential
temperature/climate (18 °C, 60 %) the drying time is 12–
characteristics according to EN 15102:2007+A1:2011,
24 hours. When applicating under extreme climatic
Decorative wall coverings – Roll and panel form.
conditions, the duration can change significantly.
2 Environmental Product Declaration - Vitrulan Textile Glass GmbH - Woven glass fibre wall covering
technique in which both sides of the unprocessed fabrics are
Base materials/Ancillary materials impregnated and then dried. The finish determines essential
Our woven glass fibre wall covering contains ca. 0.116 kg/m2 product characteristics such as stability, warp thread bonding,
glass yarns and ca. 0.029 kg/m2 coating based on starch, cutting capability, flexibility, feel, and surface roughness.
polymeric materials and inorganic additives. It is produced in Basically, the finish primes the surface optimally for subsequent
three main phases: application and painting. The finish for our pre-pigmented glass
fabrics contains high-quality white pigments – this makes
Glass fibre manufacture: The basic components of a glass painting works on the construction site highly economical and
batch are silica sand, limestone, kaolin, and boric acid. These significantly reduces labour and material costs. In the packing
components are fused at approx. 1250˚C. The molten glass area, the dried and coated fabrics are wound and shortened in
flows by gravity through the nozzles of a bushing plate made of line with customer specifications. In the packaging area, the
platinum alloy to form filaments. A surface coating called a 'size' picked rolls are packaged individually before being sent for
is applied to the individual filaments before they are gathered dispatch.
into a strand. The size largely determines the processing
characteristics of the glass fibre material. The glass filaments According to the REACH regulation, these products are
are directed across a picking roll which combines the individual considered articles which do not fall under this regulation. With
filaments as glass fibre strands before winding them on a regard to REACH, we can confirm that all raw materials we use
bobbin. These spools are then subjected to a drying process. are registered and approved for use.
The textile glass yarns are partially textured to give the fabric's
structure more volume. These products contain substances listed in the Substances of
Very High Concern candidate list (date: 15 June 2023)
Warp beam manufacture and weaving fabrics: It involves exceeding 0.1 percentage by mass: No.
attaching the textile glass yarns to fibre creels and combining
Reference service life
as warp beams. In the weaving area, gripper needle and air-jet
weaving looms generate textile glass fabric from the weft and The reference service life according to ISO 15686:1,
warp materials. This is referred to as manufacturing fabric from -2, -7 and -8 are not indicated. The product is applied on
glass yarns which are manufactured on weaving looms by internal walls and ceilings. Since it is designed to reinforce
means of crossing two thread systems. walls and ceilings, it is bonded to the building's structure. If well
maintained, there is no lifetime limitation. It creates the ideal
Coating and dispatch: In the coating area, these textile glass substrate for decorative coatings and can be repainted over
fabrics are attributed a finishing treatment that completely coats time and again without losing its performance.
the fabrics. The finish is normally applied using a special
LCA: Calculation rules
• Treatment of packaging material (A5) credits for
Declared Unit potential avoided burdens due to energy substitution of
The declared unit refers to 1 m2 of woven glass fibre wall electricity and thermal energy generation are declared in
covering with an area weight of 0.145 kg/m². module D. Installation losses are also included in this
module.
Declared unit and mass reference
Name Value Unit
End-of-Life Stage - Modules C1-C4
Declared unit 1 m2
• Mechanical dismantling is considered (C1)
Grammage 0.145 kg/m2 • Transport to EoL (C2)
Layer thickness 0.0006 m • Disposal (C4) - landfill of the glass fibre wall covering
System boundary Benefits and Loads beyond product system boundary
No credits were accounted from the EoL scenario(C4) in
Type of EPD according to EN 15804: "cradle to gate with
module D. The credits in D are solely accounting for the
options, modules C1–C4, and module D". The following
avoided burdens calculated by the inversion of electricity grid
modules are declared: A1–A3, C, D and additional modules: A4
mix and thermal energy from natural gas during packaging
+ A5.
treatment (A5).
The following life cycle stages are considered:
Geographic Representativeness
Production - Modules A1-A3
Land or region, in which the declared product system is
The product stage includes:
manufactured, used or handled at the end of the product´s
• Raw material supply (A1): glass yarns and coating lifespan: Europe
based on starch besides polymeric materials and
inorganic additives.
• Transport to the manufacturer (A2) Comparability
• Manufacturing (A3), including provision of all materials, Basically, a comparison or an evaluation of EPD data is only
products and energy, as well as waste processing up to possible if all the data sets to be compared were created
the end-of-waste state. according to EN 15804 and the building context, respectively
the product-specific characteristics of performance, are taken
Construction Stage - Modules A4- A5 into account.
The construction process stage includes: Sphera LCA FE (GaBi ts) serves as background database for
the calculation. The CUP version 2022.2 is used.
• Transport to the construction site (A4)
3 Environmental Product Declaration - Vitrulan Textile Glass GmbH - Woven glass fibre wall covering
LCA: Scenarios and additional technical information
comes with a water-activatable adhesive which is already
Characteristic product properties of biogenic carbon applied to the wall covering's backing – this adhesive then can
For 1 m2 of woven wall covering, the biogenic carbon content is be easily activated by water using the 'Aqua-Quick device'
declared below: specially developed for this purpose. Vitrulan's Aqua
Technology facilitates work and reduces processing times for
Information on describing the biogenic carbon content at
the user. The Public annexe to the EPD for the aqua technology
factory gate
is declared in an attachment.
Name Value Unit
Name Value Unit
Biogenic carbon content in product (coating kg
0.00568 Material loss (Cuttings waste at installation) 0.00654 kg
based on starch) C
Cardboard (waste packaging to incineration) 0.0121 kg/m2
Biogenic carbon content in accompanying kg
0.00912
packaging C Wooden pallets (waste packaging to
0.00799 kg/m2
incineration)
Note: 1 kg of biogenic carbon is equivalent to 44/12 kg of CO .
2 Polyethylene film (waste packaging to
0.00115 kg/m2
incineration)
Paper (waste packaging to incineration) 0.000154kg/m2
Transport to the building site (A4)
Name Value Unit
End of life (C1-C4)
Litres of fuel 0.000338 l/100km
Name ValueUnit
Transport distance 100 km
Collected separately waste type wall covering(send
Capacity utilisation (including empty runs) 50 % 0.145 kg
to landfill)
Gross weight of products transported 0.145 kg
Reuse, recovery and/or recycling potentials (D), relevant
scenario information
Installation into the building (A5) For the thermal and electrical energy generated in Module A5
The environmental results cover the cutting losses during due to the packaging treatment, avoided burdens have been
installation. The wall covering can come with/without aqua calculated by the inversion of electricity grid mix and thermal
technology (self-adhesive layers). During application, the wall energy from natural gas, using European datasets and grouped
or ceiling is pasted and then the strip of wall covering is hung to Module D.
on the prepared paste bed, or, alternatively, the wall covering
4 Environmental Product Declaration - Vitrulan Textile Glass GmbH - Woven glass fibre wall covering
LCA: Results
The following table depicts the results of the indicators concerning the estimated impact, use of resources as well as waste and other
output flows in relation to 1 m² of woven wall covering with the weight of 0.145 kg/m2.
DESCRIPTION OF THE SYSTEM BOUNDARY (X = INCLUDED IN LCA; MND = MODULE OR INDICATOR NOT DECLARED; MNR
= MODULE NOT RELEVANT)
Benefits and
Construction loads beyond
Product stage Use stage End of life stage
process stage the system
boundaries
la ire ta m w a Ry lp p u s tro p s n a rT g n iru tc a fu n a M e h t m o rf tro p s n a rTe tis e h t o t e ta g y lb m e s s A e s U e c n a n e tn ia M ria p e R tn e m e c a lp e R tn e m h s ib ru fe R y g re n e la n o ita re p Oe s u re ta w la n o ita re p Oe s u n o itc u rts n o c -e Dn o itilo m e d tro p s n a rT g n is s e c o rp e ts a W la s o p s iD -e s u e R-y re v o c e R-g n ilc y c e Rla itn e to p
A1 A2 A3 A4 A5 B1 B2 B3 B4 B5 B6 B7 C1 C2 C3 C4 D
X X X X X MND MND MNR MNR MNR MND MND X X X X X
RESULTS OF THE LCA - ENVIRONMENTAL IMPACT according to EN 15804+A2: 1 m2 Woven glass fibre wall covering
Parameter Unit A1-A3 A4 A5 C1 C2 C3 C4 D
GWP-total kg CO 2 eq 7.04E-01 1.04E-03 7E-02 1.49E-03 6.13E-04 0 2.3E-02 -6.46E-03
GWP-fossil kg CO 2 eq 7.52E-01 1.03E-03 3.86E-02 1.48E-03 6.06E-04 0 2.16E-03 -6.42E-03
GWP-biogenic kg CO 2 eq -4.74E-02 4.31E-06 3.14E-02 1.33E-05 2.54E-06 0 2.08E-02 -3.29E-05
GWP-luluc kg CO 2 eq 2.44E-04 7.05E-06 1.19E-05 3.13E-07 4.16E-06 0 3.98E-06 -7.07E-07
ODP kg CFC11 eq 3.8E-12 1.03E-16 1.76E-13 2.17E-14 6.07E-17 0 5.07E-15 -4.35E-14
AP mol H+ eq 3.63E-03 1.13E-06 1.73E-04 3.25E-06 7.3E-07 0 1.53E-05 -8.46E-06
EP-freshwater kg P eq 5.4E-06 3.74E-09 2.46E-07 4.32E-09 2.21E-09 0 3.65E-09 -8.85E-09
EP-marine kg N eq 7.85E-04 3.55E-07 3.84E-05 7.29E-07 2.43E-07 0 3.91E-06 -2.29E-06
EP-terrestrial mol N eq 8.43E-03 4.27E-06 4.19E-04 7.65E-06 2.89E-06 0 4.3E-05 -2.46E-05
kg NMVOC
POCP 2.23E-03 9.66E-07 1.08E-04 1.97E-06 6.34E-07 0 1.19E-05 -6.42E-06
eq
ADPE kg Sb eq 1.62E-07 1.05E-10 7.45E-09 4.03E-10 6.23E-11 0 2.21E-10 -9.71E-10
ADPF MJ 1.24E+01 1.37E-02 5.73E-01 2.69E-02 8.11E-03 0 2.82E-02 -1.09E-01
m3 world eq
WDP 1.02E-01 1.17E-05 8.78E-03 3.38E-04 6.91E-06 0 2.36E-04 -6.85E-04
deprived
GWP = Global warming potential; ODP = Depletion potential of the stratospheric ozone layer; AP = Acidification potential of land and water; EP =
Eutrophication potential; POCP = Formation potential of tropospheric ozone photochemical oxidants; ADPE = Abiotic depletion potential for non-fossil
resources; ADPF = Abiotic depletion potential for fossil resources; WDP = Water (user) deprivation potential)
RESULTS OF THE LCA - INDICATORS TO DESCRIBE RESOURCE USE according to EN 15804+A2: 1 m2 Woven glass fibre
wall covering
Parameter Unit A1-A3 A4 A5 C1 C2 C3 C4 D
PERE MJ 2.31E+00 9.52E-04 4.5E-01 1.49E-02 5.62E-04 0 4.24E-03 -3.01E-02
PERM MJ 3.28E-01 0 -3.28E-01 0 0 0 0 0
PERT MJ 2.64E+00 9.52E-04 1.22E-01 1.49E-02 5.62E-04 0 4.24E-03 -3.01E-02
PENRE MJ 1.24E+01 1.38E-02 6.23E-01 2.69E-02 8.14E-03 0 2.83E-02 -1.09E-01
PENRM MJ 4.95E-02 0 -4.95E-02 0 0 0 0 0
PENRT MJ 1.24E+01 1.38E-02 5.73E-01 2.69E-02 8.14E-03 0 2.83E-02 -1.09E-01
SM kg 9.57E-03 0 4.33E-04 0 0 0 0 0
RSF MJ 0 0 0 0 0 0 0 0
NRSF MJ 0 0 0 0 0 0 0 0
FW m3 4.89E-03 1.1E-06 3.2E-04 1.42E-05 6.49E-07 0 7.18E-06 -2.89E-05
PERE = Use of renewable primary energy excluding renewable primary energy resources used as raw materials; PERM = Use of renewable primary
energy resources used as raw materials; PERT = Total use of renewable primary energy resources; PENRE = Use of non-renewable primary energy
excluding non-renewable primary energy resources used as raw materials; PENRM = Use of non-renewable primary energy resources used as raw
materials; PENRT = Total use of non-renewable primary energy resources; SM = Use of secondary material; RSF = Use of renewable secondary fuels;
NRSF = Use of non-renewable secondary fuels; FW = Use of net fresh water
RESULTS OF THE LCA – WASTE CATEGORIES AND OUTPUT FLOWS according to EN 15804+A2:
1 m2 Woven glass fibre wall covering
Parameter Unit A1-A3 A4 A5 C1 C2 C3 C4 D
HWD kg 4.21E-07 7.29E-14 1.91E-08 2.32E-12 4.31E-14 0 1.45E-12 -1.48E-11
NHWD kg 6.05E-02 2.25E-06 9.99E-03 2.02E-05 1.33E-06 0 1.45E-01 -5.53E-05
RWD kg 4.95E-04 2.56E-08 2.3E-05 4.29E-06 1.51E-08 0 3.14E-07 -8.62E-06
CRU kg 0 0 0 0 0 0 0 0
MFR kg 0 0 0 0 0 0 0 0
MER kg 0 0 0 0 0 0 0 0
EEE MJ 0 0 3.03E-02 0 0 0 0 0
5 Environmental Product Declaration - Vitrulan Textile Glass GmbH - Woven glass fibre wall covering
EET MJ 0 0 5.42E-02 0 0 0 0 0
HWD = Hazardous waste disposed; NHWD = Non-hazardous waste disposed; RWD = Radioactive waste disposed; CRU = Components for re-use;
MFR = Materials for recycling; MER = Materials for energy recovery; EEE = Exported electrical energy; EET = Exported thermal energy
RESULTS OF THE LCA – additional impact categories according to EN 15804+A2-optional:
1 m2 Woven glass fibre wall covering
Parameter Unit A1-A3 A4 A5 C1 C2 C3 C4 D
Disease
PM 4E-08 7.92E-12 1.86E-09 2.69E-11 4.86E-12 0 1.88E-10 -7.01E-11
incidence
IR kBq U235 eq 5.34E-02 3.86E-06 2.5E-03 7.27E-04 2.28E-06 0 3.49E-05 -1.46E-03
ETP-fw CTUe 3.8E+00 9.73E-03 1.78E-01 1.18E-02 5.75E-03 0 1.58E-02 -2.4E-02
HTP-c CTUh 4.86E-10 2.01E-13 2.24E-11 3.38E-13 1.18E-13 0 2.42E-12 -1.1E-12
HTP-nc CTUh 4.82E-08 1.08E-11 2.21E-09 1.24E-11 6.42E-12 0 2.67E-10 -4.23E-11
SQP SQP 7.13E+00 5.81E-03 3.26E-01 9.68E-03 3.43E-03 0 5.88E-03 -1.95E-02
PM = Potential incidence of disease due to PM emissions; IR = Potential Human exposure efficiency relative to U235; ETP-fw = Potential comparative
Toxic Unit for ecosystems; HTP-c = Potential comparative Toxic Unit for humans (cancerogenic); HTP-nc = Potential comparative Toxic Unit for humans
(not cancerogenic); SQP = Potential soil quality index
Disclaimer 1 – for the indicator “Potential Human exposure efficiency relative to U235”. This impact category deals mainly with the
eventual impact of low-dose ionizing radiation on human health of the nuclear fuel cycle. It does not consider effects due to possible
nuclear accidents, occupational exposure or radioactive waste disposal in underground facilities. Potential ionizing radiation from the
soil, radon and from some construction materials is also not measured by this indicator.
Disclaimer 2 – for the indicators “abiotic depletion potential for non-fossil resources”, “abiotic depletion potential for fossil resources”,
“water (user) deprivation potential, deprivation-weighted water consumption”, “potential comparative toxic unit for ecosystems”,
“potential comparative toxic unit for humans – cancerogenic”, “Potential comparative toxic unit for humans - not cancerogenic”,
“potential soil quality index”. The results of this environmental impact indicator shall be used with care as the uncertainties on these
results are high as there is limited experience with the indicator.
References
Standards ISO 15686
ISO 15686:1, -2, -7 and -8, Buildings and constructed assets —
EN 12149 Service life planning
DIN EN 12149, Wallcoverings in roll form - Determination of
migration of heavy metals and certain other elements, of vinyl Further References
chloride monomer and of formaldehyde release
IBU 2021
EN 12524 Institut Bauen und Umwelt e.V.: General Instructions for the
DIN EN 12524:2000, Building materials and products - EPD programme of Institut Bauen und Umwelt e.V., Version
Hygrothermal properties - Tabulated design values 2.0, Berlin: Institut Bauen und Umwelt e.V., 2021, www.ibu-
epd.com
EN 12667
DIN EN 12667:2001, Thermal performance of building materials OEKO-TEX
and products - Determination of thermal resistance by means of OEKO-TEX Standard 100, label for textiles tested for harmful
guarded hot plate and heat flow meter methods - Products of substances, https://www.oeko-tex.com/en/our-
high and medium thermal resistance standards/oekotex-standard-100 (accessed on 13 July 2023)
EN 13501 PCR Part A
EN 13501-1, Fire classification of construction products and PCR - Part A: Calculation rules for the Life Cycle Assessment
building elements - Part 1: Classification using test data from and Requirements on the Background Report, version 2.1,
reaction to fire tests Institut Bauen und Umwelt e.V.,2021
EN 15804 PCR Part B
EN 15804:2012+A2:2019+AC:2021, Sustainability of PCR – Part B: Requirements of the EPD for Wall coverings, v2,
construction works — Environmental Product Declarations — Institut Bauen und Umwelt e.V., 2023
Core rules for the product category of construction products
REACH Regulation
ISO 354 REACH Regulation (EC) No 1907/2006 of the European
DIN EN ISO 354:2003, Acoustics - Measurement of sound Parliament and of the Council of 18 December 2006 concerning
absorption in a reverberation room the Registration, Evaluation, Authorisation and Restriction of
Chemicals (REACH), establishing a European Chemicals
ISO 11654 Agency, amending Directive 1999/45/EC and repealing Council
DIN EN ISO 11654:1997, Acoustics - Sound absorbers for use Regulation (EEC) No 793/93 and Commission Regulation (EC)
in buildings - Rating of sound absorption No 1488/94 as well as Council Directive 76/769/EEC and
Commission Directives 91/155/EEC, 93/67/EEC, 93/105/EC
ISO 14025 and 2000/21/EC
EN ISO 14025:2011, Environmental labels and declarations —
Type III environmental declarations — Principles and Regulation No. 305/2011
procedures Regulation (EU) No. 305/2011 of the European parliament and
of the Council of 9 March 2011 laying down harmonised
6 Environmental Product Declaration - Vitrulan Textile Glass GmbH - Woven glass fibre wall covering
conditions for the marketing of construction products and Leinfelden-Echterdingen, 2023 (https://www.gabi-
repealing Council Directive 89/106/EEC EN software.com/support/gabi)
15102:2007+A1:2011, Decorative wallcoverings - Roll and
panel form products SVHC list
Substances of Very High Concern candidate list (published in
Sphera LCA FE (GaBi ts) accordance with Article 59(10) of the REACH Regulation)
GaBi ts dataset documentation for the software system and (accessed on 13 July 2023)
databases, LBP, University of Stuttgart and thinkstep,
7 Environmental Product Declaration - Vitrulan Textile Glass GmbH - Woven glass fibre wall covering
Publisher
Institut Bauen und Umwelt e.V. +49 (0)30 3087748- 0
Hegelplatz 1 info@ibu-epd.com
10117 Berlin www.ibu-epd.com
Germany
Programme holder
Institut Bauen und Umwelt e.V. +49 (0)30 3087748- 0
Hegelplatz 1 info@ibu-epd.com
10117 Berlin www.ibu-epd.com
Germany
Author of the Life Cycle Assessment
Sphera Solutions GmbH +49 711 341817-0
Hauptstraße 111- 113 info@sphera.com
70771 Leinfelden-Echterdingen www.sphera.com
Germany
Owner of the Declaration
Vitrulan Textile Glass GmbH +49 9227 77-0
Bernecker Straße 8 info@vitrulan.com
95509 Marktschorgast www.vitrulan.com
Germany
8 Environmental Product Declaration - Vitrulan Textile Glass GmbH - Woven glass fibre wall covering
