ENVIRONMENTAL PRODUCT DECLARATION
as per ISO 14025 and EN 15804+A2
Owner of the Declaration DuPont de Nemours (Luxembourg) s.à r.l
Programme holder Institut Bauen und Umwelt e.V. (IBU)
Publisher Institut Bauen und Umwelt e.V. (IBU)
Declaration number EPD-DUP-20220321-CBA1-EN
Issue date 13.12.2022
Valid to 12.12.2027
DuPontTM Typar® / Xavan® / Plantex® / Zemdrain®
DuPont de Nemours (Luxembourg) s.à r.l
www.ibu-epd.com | https://epd-online.com
Umwelt Produktdeklaration Name des Herstellers – Name des Produkts
General Information
DuPont de Nemours (Luxembourg) s.à r.l DuPontTM Typar® / Xavan® / Plantex® /
Zemdrain®
Programme holder Owner of the declaration
IBU – Institut Bauen und Umwelt e.V.
Hegelplatz 1 DuPont de Nemours (Luxembourg) s.à.r.l.
10117 Berlin Rue Général Patton
Germany L-2984 Contern
Luxembourg
Declaration number Declared product / declared unit
EPD-DUP-20220321-CBA1-EN 1 m2 DuPontTM Typar®
This declaration is based on the product Scope:
category rules:
Technical Textiles, 2013 This document applies to the whole of DuPontTM
(PCR checked and approved by the SVR) Typar® products manufactured in DuPont de Nemours
(Luxembourg) s.à.r.l.
Issue date The declared unit weight is 100 g/m2.
13.12.2022 LCA data were compiled using production data for the
year 2021. The declaration holder is responsible for the
Valid to underlying data and its verification.
12.12.2027
The owner of the declaration shall be liable for the
underlying information and evidence; the IBU shall not
be liable with respect to manufacturer information, life
cycle assessment data and evidences.
The EPD was created according to the specifications
of EN 15804+A2. In the following, the standard will be
simplified as EN 15804.
Verification
The standard EN 15804 serves as the core PCR
Independent verification of the declaration and data
according to ISO 14025:2011
Dipl. Ing. Hans Peters internally x externally
(chairman of Institut Bauen und Umwelt e.V.)
Dr. Alexander Röder Vito D'Incognito
(Managing Director Institut Bauen und Umwelt e.V.)) (Independent verifier)
Product
Product description/Product definition
DuPont™ Typar® is composed of thermally bonded EN 13249:2016/ Roads and other trafficked areas
continuous polypropylene filaments. (excluding railways and asphalt inclusion)
DuPont™ Typar® serves different markets with EN 13250:2016/ Railways
different functions and can be sold under different EN 13251:2016/ Earthworks, foundations and retaining
brand names in function of the application (Typar®, structures
Xavan®, Plantex® and Zemdrain®). EN 13252:2016/ Drainage systems
For ease of reading, only Typar® will be used hereafter EN 13253:2016/ Erosion control works (coastal
protection, bank revetments)
Only for Typar® products carrying a CE Marking: EN 13254:2016/ Reservoirs and dams
EN 13255:2016/ Canals
EU regulation no. /305/2011/ (CPR) applies for putting EN 13256:2016/ Tunnels and underground structures
the product on the market in the EU/EFTA (with the EN 13257:2016/ Solid waste disposal sites
exception of Switzerland). This product requires a EN 13265:2016/ Liquid waste containment projects
declaration of performance taking into account the
following standards relating to required characteristics
for geotextiles and CE labelling.
2 Environmental Product Declaration DuPont de Nemours (s.à r.l.) – DuPont™ Typar®
Application Constructional data
Name Value Unit
DuPont™ Typar® is used as geosynthetics in civil Mass per unit area EN ISO 9864 30 - 400 g/m2
engineering (as a geotextile, filter for composite drains, Thickness (2kPa) EN ISO 9863-1 0.30 -0.90 mm
and concrete lining products): its functions are Tensile strength MD/XD EN
90-1300 N/50mm
separation, filtration, protection, and controlled 29073-3
permeability formwork liner. Elongation MD/XD (%) EN 29073-
30-60 %
In construction, DuPont™ Typar® is used as a 3
substrate in composite sheet structures such as
coatings, laminates.
Typar® products also serve other markets and
applications such as:
-Landscape: weed control, root control and soil Base materials/Ancillary materials
stabilization.
-Filtration (liquid filtration, air filtration, masks): Typar® is a high strength spunbond nonwoven fabric
substrate, carrier, and protection layer for filter made of thermally bonded (endless) polypropylene
medium. filaments.
-Primary carpet backing and reinforcement for Polypropylene is thus the main material of the product
footwear. (99 % on average), while a small amount of additives
(1 %) are added to give specific properties.
Technical Data This product/at least one partial article contains
For the products carrying a CE Marking, the product’s substances listed in the candidate list (date:
performance values comply with the declaration of 10.06.2022) exceeding 0.1 percentage by mass: no
performance in relation to its main features in
accordance with the following European standards: This product/article/at least one partial article contains
other CMR substances in categories 1A or 1B which
EN 13249:2016/ Roads and other trafficked areas are not on the candidate list, exceeding 0.1 percentage
(excluding railways and asphalt inclusion) by mass: no
EN 13250:2016/ Railways
EN 13251:2016/ Earthworks, foundations and retaining Biocide products were added to this construction
structures product or it has been treated with biocide products
EN 13252:2016/ Drainage systems (this then concerns a treated product as defined by the
EN 13253:2016/ Erosion control works (coastal (EU) Ordinance on Biocide Products No. 528/2012): no
protection, bank revetments)
EN 13254:2016/ Reservoirs and dams
EN 13255:2016/ Canals Reference service life
EN 13256:2016/ Tunnels and underground structures The service life of Typar® depends on the application
EN 13257:2016/ Solid waste disposal sites and whether it is covered or not.
EN 13265:2016/ Liquid waste containment projects In geotextile applications, Typar® product are predicted
to be durable for 100 years in natural soils with 4 ≤ pH
≤ 9 and soil temperatures ≤ 25°C.
LCA: Calculation rules
Declared Unit The product is manufactured in Luxembourg. All
The declared unit is 1 m² of geotextile. Its mass per energy and materials flows were considered. Only a
unit of area in accordance with /EN ISO 9864/ is 30 to few material flows were excluded from the modelling,
400 g/m². A surface weight of 100 g/m² has been used but the sum of their weight did not exceed 1 % of the
when calculating the lifecycle analysis for this EPD. total input mass. Manufacturing of the production
machines and systems and associated infrastructure
To calculate the specific impacts of a Typar® product, were not taken into account for the life cycle
the EPD results need to be multiplied by the ratio assessment.
between its specific grammage and 100 g/m2. The
variations for DuPont™ Typar® is thus proportional to Transport to the construction site (A4) was based on
the variations of the grammage (factor of 13 between European market shares of 2021 at country level,
the minimum and maximum value). provided by DuPont Luxembourg s.à.r.l., to cover at
least 90 % of the sales. Eurostat data representative of
Declared unit 2019 were used to model the shares between the
Name Value Unit packaging disposal routes during the installation into
Declared unit 1 m2 the building (A5).
Mass per unit area EN ISO 9864 100 g/m2
Thickness (2kPa) EN ISO 9863-1 0.40 mm Regarding background data, the Luxembourg
electricity grid mix were applied to the production plant.
Primary production data were collected to model the Other background data were specific to Germany or
production process (A1-A3), and are representative of the European average and were not older than 10
the year 2021.
3 Environmental Product Declaration DuPont de Nemours (s.à r.l.) – DuPont™ Typar®
years. Some proxies were used for the modelling of · A1-A3: Manufacturing of pre-products,
additives. packaging, ancillary materials, transport to the factory
The representativeness can be classified as very good and production, with the associated energy supply and
for all the foreground data, and for most of the waste handling
background data. · A4: Transport to the construction site
· A5: Installation into the building including
The GaBi database (Sphera Solutions GmbH, 2022.1) disposal of packaging
was used to model background data. · C4: Waste disposal, namely landfill
Comparability
Basically, a comparison or an evaluation of EPD data
System boundary is only possible if all the data sets to be compared
Type of EPD: Cradle-to-gate (with options) were created according to EN 15804 and the building
The system boundaries of the EPD follow the modular context, respectively the product-specific
construction system as described by EN 15804. characteristics of performance, are taken into account.
The LCA considers the following modules:
LCA: Scenarios and additional technical information
Characteristic product properties
Information on biogenic carbon
The product does not contain biogenic carbon.
Information on describing the biogenic Carbon
Content at factury gate
Name Value Unit
Biogenic Carbon Content in
0.0007 kg C
accompanying packaging
Transport to the building site (A4)
Name Value Unit
Transport distance (truck) 854 km
Transport distance (container
6 km
ship)
Installation into the building (A5)
Name Value Unit
Cardboard/paper waste to landfill 2.48E-04 kg
Cardboard/paper waste to
2.65E-04 kg
incineration
Plastic waste to landfill 5.52E-05 kg
Plastic waste to incineration 8.80E-5 kg
End of life (C1-C4)
Name Value Unit
Collected as mixed construction
0.1 kg
waste
Landfilling 0.1 kg
4 Environmental Product Declaration DuPont de Nemours (s.à r.l.) – DuPont™ Typar®
LCA: Results
The results displayed below apply to 1 m2 of DuPont™ Typar® product, with a declared unit weight of 100 g/m2.
DESCRIPTION OF THE SYSTEM BOUNDARY (X = INCLUDED IN LCA; ND = MODULE OR INDICATOR NOT
DECLARED; MNR = MODULE NOT RELEVANT)
BENEFITS AND
CONSTRUCTI LOADS
PRODUCT STAGE ON PROCESS USE STAGE END OF LIFE STAGE BEYOND THE
STAGE SYSTEM
BOUNDARIES
5 Environmental Product Declaration DuPont de Nemours (s.à r.l.) – DuPont™ Typar®
lairetam
waR
ylppus tropsnarT
gnirutcafunaM
eht
morf
tropsnarT
etis
eht
ot
etag
ylbmessA esU
ecnanetniaM
riapeR
tnemecalpeR tnemhsibrufeR
ygrene
lanoitarepO esu
retaw
lanoitarepO esu
noitcurtsnoc-eD
noitilomed tropsnarT
gnissecorp
etsaW
lasopsiD -esueR -yrevoceR -gnilcyceR laitnetop
A1 A2 A3 A4 A5 B1 B2 B3 B4 B5 B6 B7 C1 C2 C3 C4 D
X X X X X ND ND MNR MNR MNR ND ND ND ND ND X ND
RESULTS OF THE LCA - ENVIRONMENTAL IMPACT according to EN 15804+A2: 1 m2 DuPont™ Typar®
Core Indicator Unit A1-A3 A4 A5 C4
Global warming potential - total [kg CO2-Eq.] 4.51E-1 7.48E-3 9.71E-4 7.02E-3
Global warming potential - fossil fuels [kg CO2-Eq.] 4.51E-1 7.31E-3 2.51E-4 7.09E-3
Global warming potential - biogenic [kg CO2-Eq.] 7.50E-4 1.22E-4 7.20E-4 -7.54E-5
GWP from land use and land use change [kg CO2-Eq.] 5.19E-5 4.15E-5 1.47E-8 3.45E-6
Depletion potential of the stratospheric ozone layer [kg CFC11-Eq.] 1.35E-12 4.47E-16 1.10E-16 9.52E-15
Acidification potential, accumulated exceedance [mol H+-Eq.] 2.47E-3 4.45E-5 2.31E-7 2.10E-5
Eutrophication, fraction of nutrients reaching freshwater
[kg P-Eq.] 9.84E-6 2.22E-8 2.73E-9 1.32E-6
end compartment
Eutrophication, fraction of nutrients reaching marine end
[kg N-Eq.] 3.39E-4 2.18E-5 1.00E-7 4.65E-6
compartment
Eutrophication, accumulated exceedance [mol N-Eq.] 3.66E-3 2.42E-4 9.40E-7 5.10E-5
Formation potential of tropospheric ozone photochemical
[kg NMVOC-Eq.] 1.02E-3 4.13E-5 3.17E-7 1.49E-5
oxidants
Abiotic depletion potential for non-fossil resources [kg Sb-Eq.] 3.20E-8 6.23E-10 3.47E-12 4.92E-10
Abiotic depletion potential for fossil resources [MJ] 1.00E+1 9.96E-2 5.00E-4 1.01E-1
Water (user) deprivation potential, deprivation-weighted [m³ world-Eq
1.51E-1 6.68E-5 6.87E-5 -6.99E-5
water consumption (WDP) deprived]
RESULTS OF THE LCA - INDICATORS TO DESCRIBE RESOURCE USE according to EN 15804+A2: 1 m2
DuPont™ Typar®
Indicator Unit A1-A3 A4 A5 C4
Renewable primary energy as energy carrier [MJ] 7.21E-1 5.66E-3 8.33E-3 4.56E-6
Renewable primary energy resources as material utilization [MJ] 3.59E-4 3.02E-14 8.58E-13 4.72E-16
Total use of renewable primary energy resources [MJ] 7.21E-1 5.66E-3 8.33E-3 4.56E-6
Non-renewable primary energy as energy carrier [MJ] 1.00E+1 9.98E-2 1.01E-1 5.55E-5
Non-renewable primary energy as material utilization [MJ] 1.79E-4 3.50E-6 1.38E-6 7.54E-10
Total use of non-renewable primary energy resources [MJ] 1.00E+1 9.99E-2 1.01E-1 5.55E-5
Use of secondary material [kg] 3.23E-3 0.00E+0 0.00E+0 0.00E+0
Use of renewable secondary fuels [MJ] 1.07E-7 0.00E+0 0.00E+0 0.00E+0
Use of non-renewable secondary fuels [MJ] 9.87E-9 0.00E+0 0.00E+0 0.00E+0
Use of net fresh water [m³] 3.93E-3 6.40E-6 1.63E-6 1.30E-6
RESULTS OF THE LCA – WASTE CATEGORIES AND OUTPUT FLOWS according to EN 15804+A2:
1 m2 DuPont™ Typar®
Indicator Unit A1-A3 A4 A5 C4
Hazardous waste disposed [kg] 2.87E-10 4.78E-13 6.52E-14 1.55E-11
Non-hazardous waste disposed [kg] 1.03E-3 1.43E-5 2.69E-4 9.96E-2
Radioactive waste disposed [kg] 1.28E-4 1.23E-7 1.33E-8 1.24E-6
Components for re-use [kg] 0.00 0.00 0.00 0.00
Materials for recycling [kg] 0.00 0.00 0.00 0.00
Materials for energy recovery [kg] 0.00 0.00 0.00 0.00
Exported electrical energy [MJ] 0.00E+0 0.00E+0 9.68E-4 0.00E+0
Exported thermal energy [MJ] 0.00E+0 0.00E+0 1.74E-3 0.00E+0
RESULTS OF THE LCA – additional impact categories according to EN 15804+A2-optional:
1 m2 DuPont™ Typar®
Indicator Unit A1-A3 A4 A5 C4
Potential incidence of disease due to PM emissions [Disease
ND ND ND ND
Incidence]
Potential Human exposure efficiency relative to U235 [kBq U235-
ND ND ND ND
Eq.]
Potential comparative toxic unit for ecosystems [CTUe] ND ND ND ND
Potential comparative toxic unit for humans - cancerogenic [CTUh] ND ND ND ND
Potential comparative toxic unit for humans - not cancerogenic [CTUh] ND ND ND ND
Potential soil quality index [-] ND ND ND ND
Disclaimer 1 – for the indicator “Potential Human exposure efficiency relative to U235”.
This impact category deals mainly with the eventual impact of low dose ionizing
radiation on human health of the nuclear fuel cycle. It does not consider effects due to possible
nuclear accidents, occupational exposure nor due to radioactive waste disposal in underground
facilities. Potential ionizing radiation from the soil, from radon and from some construction materials is also not
measured by this indicator.
Disclaimer 2 – for the indicators “abiotic depletion potential for non-fossil resources”, “abiotic depletion potential
for fossil resources”, “water (user) deprivation potential, deprivation-weighted water consumption”, “potential
comparative toxic unit for ecosystems”, “potential comparative toxic unit for humans – cancerogenic”, “Potential
comparative toxic unit for humans - not cancerogenic”, “potential soil quality index”.
The results of this environmental impact indicator shall be used with care as the
uncertainties on these results are high or as there is limited experienced with the indicator.
References
EN 13249 EN 15804:2012+A2:2019+AC:2021, Sustainability of
EN 13249:2016, Geotextiles and geotextile-related construction works — Environmental Product
products - Characteristics required for use in the Declarations — Core rules for the product category of
construction of roads and other trafficked areas construction products.
(excluding railways and asphalt inclusion).
EN 29073-3
EN 13250 EN 29073-3:1992, Textile; test method for nonwovens;
EN 13250:2016, Geotextiles and geotextile-related Part 3: Determination of tensile strength and
products - Characteristics required for use in the elongation
construction of railways.
ISO 14025
EN 13251 EN ISO 14025:2011, Environmental labels and
EN 13251:2016, Geotextiles and geotextile-related declarations — Type III environmental declarations —
products - Characteristics required for use in Principles and procedures.
earthworks, foundations and retaining structures.
EN ISO 9863-1
EN 13252 EN ISO 9863-1:2016/A1:2019, Geosynthetics -
EN 13252:2016, Geotextiles and geotextile-related Determination of thickness at specified pressures -
products - Characteristics required for use in drainage Part 1: Single layers
systems.
ISO 9864
EN 13253 EN ISO 9864:2005-05, Geosynthetics - Test method
EN 13253:2016, Geotextiles and geotextile-related for the determination of mass per unit area of
products - Characteristics required for use in erosion geotextiles and geotextile-related products.
control works (coastal protection, bank revetments).
EN 13254 Further References
EN 13254:2016, Geotextiles and geotextile-related
products - Characteristics required for the use in the GaBi software and database:2022
construction of reservoirs and dams. GaBi software/database, version 10.6.2.9. Sphera
Solutions GmbH, 2022.
EN 13255
EN 13255:2016, Geotextiles and geotextile-related IBU 2021
products - Characteristics required for use in the Institut Bauen und Umwelt e.V.: General Instructions
construction of canals. for the EPD programme of Institut Bauen und Umwelt
e.V., Version 2.0, Berlin: Institut Bauen und Umwelt
EN 13256 e.V., 2021. www.ibu-epd.com
EN 13256:2016 Geotextiles and geotextile-related
products - Characteristics required for use in the PCR 2021, Part A
construction of tunnels and underground structures. PCR Guidance-Texts for Building-Related Products
and Services: Calculation Rules for the Life Cycle
EN 13257 Assessment and Requirements on the Project Report
EN 13257:2016, Geotextiles and geotextile-related according to EN 15804+A2:2019
products - Characteristics required for use in solid
waste disposals. PCR 2013, Part B
Part B - PCR Guidance-Texts for Building-Related
EN 13265 Products and Services: Requirements on the EPD for
EN 13265:2016, Geotextiles and geotextile-related Technical Textiles (version 1.0, 2013)
products - Characteristics required for use in liquid
waste containment projects. DuPont™, the DuPont Oval Logo, and all trademarks
and service marks denoted with ™, SM or ® are
EN 15804
6 Environmental Product Declaration DuPont de Nemours (s.à r.l.) – DuPont™ Typar®
owned by affiliates of DuPont de Nemours, Inc. unless
otherwise noted.
7 Environmental Product Declaration DuPont de Nemours (s.à r.l.) – DuPont™ Typar®
Publisher
Institut Bauen und Umwelt e.V. Tel +49 (0)30 3087748- 0
Hegelplatz 1 Fax +49 (0)30 3087748- 29
10117 Berlin Mail info@ibu-epd.com
Germany Web www.ibu-epd.com
Programme holder
Institut Bauen und Umwelt e.V. Tel +49 (0)30 - 3087748- 0
Hegelplatz 1 Fax +49 (0)30 – 3087748 - 29
10117 Berlin Mail info@ibu-epd.com
Germany Web www.ibu-epd.com
Author of the Life Cycle
Assessment Tel 00352-275888-1
Luxembourg Institute of Science Fax 00352-275888-555
and Technology (LIST) Mail info@list.lu
Avenue des Hauts-Fourneaux 5 Web www.list.lu
4362 Esch/Alzette
Luxembourg
Owner of the Declaration
DuPont de Nemours (Luxembourg) Tel +352 3666 5210
s.à r.l. Fax +352 3666 0000
Rue Général Patton 1 Mail tyvek.info@dupont.com
2984 Contern Web www.dupont.com
Luxembourg
