ENVIRONMENTAL PRODUCT DECLARATION
as per ISO 14025 and EN 15804+A2
Owner of the Declaration ARGE – The European Federation of Locks and Building Hardware Manufacturers
Publisher Institut Bauen und Umwelt e.V. (IBU)
Programme holder Institut Bauen und Umwelt e.V. (IBU)
Declaration number EPD-ARG-20230541-IBG1-EN
Issue date 02.04.2024
Valid to 01.04.2029
Hinges
ARGE – The European Federation of Locks
and Building Hardware Manufacturers
This EPD is valid only for products supplied by an ARGE EPD licence holder.
www.ibu-epd.com | https://epd-online.com
1. General Information
ARGE – The European Federation of Locks Hinges
and Building Hardware Manufacturers
Programme holder Owner of the declaration
IBU – Institut Bauen und Umwelt e.V. ARGE – The European Federation of Locks and Building Hardware
Hegelplatz 1 Manufacturers
10117 Berlin Offerstraße 12
Germany 42551 Velbert
Germany
Declaration number Declared product / declared unit
EPD-ARG-20230541-IBG1-EN 1 kg of hinge
This declaration is based on the product category rules: Scope:
Building Hardware products, 01.08.2021 This ARGE EPD covers products used to enable doors and windows in
(PCR checked and approved by the SVR) buildings to pivot about a fixed axis in the case of single-axis hinges, and
about an axis which is movable in space in the case of multi-axis, in
particular concealed hinges. The reference product used to calculate the
Issue date impact this product group has on the environment is a single-axis hinge
composed primarily of Zamak, steel and aluminium, and has been selected
02.04.2024
for the LCA (Life Cycle Assessment) because it is the product with the
highest impact for 1 kg of product. A validity scope analysis has also been
carried out to determine the limiting factors for hinges covered by this EPD.
Valid to
In a preliminary study (simplified LCA), it has been confirmed that this EPD
01.04.2029 represents the worst-case condition and it can therefore be used to cover
all hinges manufactured in Europe by ARGE member companies.
The owner of the declaration shall be liable for the underlying information
and evidence; the IBU shall not be liable with respect to manufacturer
information, life cycle assessment data and evidences.
The EPD was created according to the specifications of EN 15804+A2. In
the following, the standard will be simplified as EN 15804.
Verification
The standard EN 15804 serves as the core PCR
Independent verification of the declaration and data according to ISO
Dipl.-Ing. Hans Peters
14025:2011
(Chairman of Institut Bauen und Umwelt e.V.)
internally X externally
Florian Pronold Dr. Matthew Fishwick,
(Managing Director Institut Bauen und Umwelt e.V.) (Independent verifier)
1 Environmental Product Declaration - ARGE – The European Federation of Locks and Building Hardware Manufacturers - Hinges
2. Product
larger quantity of hinges, as they are marketed as "B2B"
2.1 Product description/Product definition
products and not to end-users.
This EPD covers products used to enable doors and windows
in buildings to pivot about a fixed axis in the case of single-axis 2.5 Base materials/Ancillary materials
hinges, and about an axis moveable in space in the case of Composition of product analysed for this EPD:
multi-axis hinges, in particular concealed hinges – including
hinges with a spring action. For the placing on the market of the The values given in the table below are for the product
product in the European Union/European Free Trade analysed for this EPD. Ranges of values for other products
Association (EU/EFTA) (with the exception of Switzerland) covered by the validity scope analysis are shown in brackets.
Regulation (EU) No. 305/2011 (CPR) applies, with the Name Value Unit
exception of spring hinges. Single-axis hinges need a
Zamak (0.00% – 74.06%) 74.1 %
declaration of performance taking into consideration EN
Steel (0.00% – 98.90%) 17.3 %
1935:2002+AC:2003, Building hardware - Single-axis hinges -
Requirements and test methods and the CE-marking. Aluminium (0.00% – 41.46%) 8.65 %
Multi-axis concealed hinges may voluntarily be CE-marked Stainless steel (0.00% – 52.89%) 0 %
according to EAD 020001-01-0405, dated March 2017, Multi- Nylon 6 (0.00% – 5.65%) 0 %
axis concealed hinge assemblies, and if voluntarily CE-marked
Zamak is an alloy with a base metal of zinc and alloying
shall have a declaration of performance.
elements of aluminium, magnesium, and copper. Components
made of Zamak are die-cast.
For the application and use the respective national provisions
at the place of use apply.
Steel is produced by combining iron with carbon as well as
2.2 Application other elements depending on the desired characteristics.
These products are designed to be integrated into door and Components made of steel are formed by stamping or other
window assemblies consisting of various materials and used for types of mechanical processing.
various applications. Their purpose is to provide the door or
window with the means to pivot about a fixed axis in the case of Aluminium is a non-ferrous metal produced from bauxite by
single-axis hinges, and about an axis moveable in space in the the Bayer process. Components made of aluminium are
case of multi-axis hinges, in particular concealed hinges – manufactured by extrusion or other types of mechanical
including hinges with a spring action. These different types of processing.
hinges may be used for interior and exterior doors as well as for
windows. Stainless steel is produced by combining iron with chromium
as well as other elements depending on the desired
2.3 Technical Data characteristics. Components made of steel are formed by
Ideally, products should comply with a suitable technical stamping or other types of mechanical processing.
specification. EN 1935 is an example of such a specification for
single-axis hinges and some products will comply with it. EAD Nylon 6 is a polymer, in particular polyamide. It is formed by
020001-01-0405 is an example of such a specification for multi- the ring-opening polymerisation of caprolactam. Components
axis, concealed hinges and some products will comply with it. In made of Nylon 6 are formed by injection moulding or other
both cases, the relevant grading structure is as shown in the thermal forming processes.
following table:
Name Value Unit 1) This product/article/at least one partial article contains
Category of use 1 - 4 Grade substances listed in the ECHA candidate list (date: 14.06.2023)
exceeding 0.1 percentage by mass: Certain components may
3, 4,
Durability Grade contain small amounts of lead (CAS no. 7439-92-1) as an
7
alloying element.
Test door mass 0 - 7 Grade
Suitability for fire resistance & smoke control 2) This product/article/at least one partial article contains other
0, 1 Grade
doors cancerogenic, mutagenic, reprotoxic (CMR) substances in
Safety 1 Grade categories 1A or 1B which are not on the ECHA candidate list,
Corrosion resistance 0 - 5 Grade exceeding 0.1 percentage by mass: no.
Security – burglar resistance 0 , 1 Grade
3) Biocide products were added to this construction product or it
Hinge grade 1 - 14 Grade
has been treated with biocide products (this then concerns a
Performance data of the product in accordance with the treated product as defined by the (EU) Ordinance on Biocide
declaration of performance with respect to its essential Products No. 528/2012): no.
characteristics according to EN 1935:2002+AC:2003, Building
2.6 Manufacture
hardware - Single-axis hinges - Requirements and test
methods, and and EAD 020001-01-0405, Multi-axis concealed The manufacture of a hinge usually follows a 3-step process:
hinge assemblies. In case of multi-axis hinges which are not 1. Manufacture of the components: this step may include
CE-marked performance data of the product with respect to its surface treatment in the factory or by external
characteristics shall be in accordance with the relevant contractors.
technical provision. 2. Pre-assembly of modules (in the factory).
3. Final assembly (in the factory).
2.4 Delivery status
The products are sold by unit. Deliveries of individual items are 2.7 Environment and health during manufacturing
possible but are an exception. Standard deliveries comprise a
2 Environmental Product Declaration - ARGE – The European Federation of Locks and Building Hardware Manufacturers - Hinges
Regular measurements of air quality and noise levels are use and environmental conditions. It is required that installation,
carried out by the manufacturers, the ARGE member as well as maintenance of the product, must be done in line
companies. The results shall be within the mandatory safety with instructions provided by the manufacturer.
levels. In areas where employees are exposed to chemical
products, the required protective clothing and technical 2.13 Extraordinary effects
protective devices shall be provided. Regular health checks are Fire
mandatory for employees in production facilities. In general, the product is suitable for use in fire resisting and/or
smoke control door or window set according to one of the
2.8 Product processing/Installation classes in EN 1935 for single-axis hinges and EAD 020001-01-
The installation of the product may vary depending on the type 0405 for multi-axis hinges, unless it is classified in class/grade
of door or window and the specific situation, but the products 0.
shall not require energy consumption for installation.
Water
2.9 Packaging The declared product is intended to be used in buildings under
Normally, each individual product is packed in paper or normal conditions (indoor or outdoor). It shall not emit
cardboard. These individual products are then packed in a hazardous substances in the event of flooding.
cardboard box and stacked on wooden pallets for transport to
the customer. Mechanical destruction
Mechanical destruction of the declared product shall not
Waste from product packaging is collected separately for waste materially alter its composition or have any adverse effect on
disposal (including recycling). the environment.
2.10 Condition of use 2.14 Re-use phase
Once installed, the products shall require no servicing during Removal of the hinge (for re-use or recycling) shall have no
their expected service lives. There shall be no consumption of adverse effect on the environment.
water or energy linked to their use, and they do not cause any
emissions. 2.15 Disposal
Hinge components should be recycled wherever possible,
2.11 Environment and health during use providing that there is no adverse effect on the environment.
No environmental damage or health risks are to be expected The waste code in accordance with the European Waste Code
during normal conditions of use. is 17 04 07.
2.12 Reference service life 2.16 Further information
The reference service life is 30 years under normal working Details of all types and variants can be found on the
conditions. This corresponds to passing a mechanical manufacturers' websites. The respective website addresses are
endurance test of 200.000 cycles as specified in EN 1935. The available at https://arge.org.
reference service life is dependent on the actual frequency of
3. LCA: Calculation rules
A4 module represents the transport of the finished hinges to the
3.1 Declared Unit
installation site.
The declared unit for all products covered by ARGE EPD is 1 There is no waste associated with the installation of the
kg (of product). Since individual products will rarely weigh product. The A5 module therefore represents only the disposal
exactly 1 kg it is necessary to establish the exact weight of the of the product packaging.
product and then use this as a correction factor to determine The End-of-Life (EoL) stages are also considered. The
the true values for 1 kg of product in the tables (Section 5). transportation to the EoL disposal site is taken into account in
Declared unit module C2. Module C4 covers the disposal of the locks. Module
C3 covers the recycling of the individual elements according to
Name Value Unit
European averages, with the remaining waste divided between
Declared unit 1 kg
incineration and landfill.
Mass of declared product 0.613 kg Such a mixed scenario is declared due to the complex material
Raw density 1 kg/m3 mix of the product and the dependency of the EoL-route on the
EoL-route of the product the hinge has been integrated into.
In practice, the end of life has been modelled as follows:
3.2 System boundary • when a material is sent for recycling, generic transport
Type of the EPD: "cradle to gate with options, with modules C1 and electric consumption of a shredder is taken into
– C4, and module D (A1-A3, C1-C3, D and additional account (corresponding to the process 'Grinding,
modules)" metals'). Only then, is the material considered to have
attained the 'end-of-waste' state.
The analysis of the product life cycle includes the production • each type of waste is modelled as a transport to the
and transport of the raw materials, the manufacture of the treatment site with a distance of 30 km. Parts sent for
product and the packaging materials which are declared in recycling include electricity consumption (grinding) and
modules A1-A3. a flow ('Materials for recycling, unspecified').
Losses during production are considered as waste and are sent
3.3 Estimates and assumptions
for recycling. No recycling processes are taken into account
except for transport and electricity consumption for grinding the The LCA data of the declared hinges had been calculated by
metals. When recycled metals are used as raw material only the production data of in total 2 ARGE member companies,
their transformation process is taken into account and not the representing 6 different products. These companies had been
extraction of the raw material. chosen by ARGE as being representative by means of their
3 Environmental Product Declaration - ARGE – The European Federation of Locks and Building Hardware Manufacturers - Hinges
production processes and their market shares. The hinge entire database having been updated in 2021).
chosen as representative for this calculation follows the "worst- Geography: Data come from production sites of the ARGE
case" principle as explained under 6. LCA interpretation. member companies. Generic data come from the ecoinvent
database, representative for European production processes.
3.4 Cut-off criteria
The cut-off criteria considered are 1% of renewable and non- Technology: Material shaping technologies are based on
renewable primary energy usage and 1% of the total mass of European technology in the case of the use of generic data.
that unit process. The total neglected input flows per module
shall be a maximum of 5% of energy usage and mass. A total of 6 typical products (based on sales figures) have been
evaluated and the worst-case results are used in the tables.
For this study, all input and output flows have been considered
at 100%, including raw materials as per the product 3.7 Period under review
composition provided by the manufacturer and packaging of The data of the LCA is based on the annual production data of
raw materials as well as the final product. Energy and water an ARGE member from 2013, considered representative for the
consumptions have also been considered at 100% according to year 2022.
the data provided.
3.8 Geographic Representativeness
With the approach chosen, no significant environmental Land or region, in which the declared product system is
impacts are known to have been cut off. manufactured, used or handled at the end of the product´s
lifespan: Europe
3.5 Background data
For the life cycle modelling of the considered product, all
3.9 Allocation
relevant background datasets are taken from ecoinvent v3.8
(system model: cut-off by classification). The products are produced in numerous production sites. All
data were provided by the manufacturers of the products per
3.6 Data quality unit and then divided by the mass of the product to give a value
The objective of this evaluation is to evaluate the environmental per kg of product produced.
impacts generated by the products throughout their entire life
cycles. To this end, ISO 14040, ISO 14044 and EN 15804 have The assumptions relating to the EoL of the product are
been met regarding the quality of data on the following different described in the section System Boundaries.
criteria:
3.10 Comparability
Time: The life cycle inventory data used come from: Basically, a comparison or an evaluation of EPD data is only
possible if all the data sets to be compared were created
• Data collected specifically for this study on the ARGE
according to EN 15804 and the building context, respectively
member companies' manufacturing sites. Datasets are
the product-specific characteristics of performance, are taken
based on 1-year averaged data (time period: January
into account.
2013 to December 2013 considered representative for
2022).
ecoinvent v3.8 (system model: cut-off by classification) has
• In the absence of collected data, generic data from the
been used as the background database.
ecoinvent v3.8 database has been used. This is updated
regularly and is representative of current processes (the
4. LCA: Scenarios and additional technical information
Characteristic product properties of biogenic carbon
Reference service life
Name Value Unit
Information on the biogenic carbon content at factory gate
Reference service life 30 a
Note: 1 kg of biogenic carbon is equivalent to 44/12 kg of CO .
2
Test cycles over RSL (EN 1935) 200'000 cycles
Name Value Unit
kg End of life (C1-C4)
Biogenic carbon content in product 0
C Name Value Unit
Biogenic carbon content in accompanying kg Collected separately waste type 1 kg
0.0572
packaging C Recycling 0.251 kg
Energy recovery 0.345 kg
The following information is the basis of the declared modules Landfilling 0.404 kg
within the LCA in this EPD.
It is assumed that a 16–32-ton truck is used to transport the
Transport to the building site (A4)
product:
Name Value Unit - Transport to shredding facility for metal recovery: 150 km
Litres of fuel 25.8 l/100km - Transport to municipal waste incineration plant: 50 km
- Transport to landfill: 30 km
Transport distance 3500 km
Capacity utilisation (including empty runs) 36 %
Reuse, recovery and/or recycling potentials (D), relevant
scenario information
Installation into the building (A5)
Name Value Unit
Module D contains the benefits and loads beyond the system
Material loss 0.138 kg boundary related to the recycling of metals, which result from
4 Environmental Product Declaration - ARGE – The European Federation of Locks and Building Hardware Manufacturers - Hinges
the treatment of recycled materials from the point of end-of- quantified as the material for recycling leaving modules A1-C4
waste status to the point of substitution (as costs) and the minus the input of secondary scrap (secondary material, SM) to
substitution of primary resources (as benefits). the product system;
- in the case of brass and zinc alloys, which are composed of
According to EN 16710, clause 6.4.3.3: 'In module D two different constituting metals, no difference shall be made
substitution effects are calculated only for the resulting net between the input of secondary constituting metals (Cu and Zn;
output flow. Cu and Sn) and its alloys (CuZn; CuSn).
For building hardware, the following rules apply for the Negative net output flows have not been considered in the
quantification of net output flows: quantification of module D.
- all production scrap and cuttings leave modules A1-B3 as
sorted scrap without allocated burdens from primary production; It also includes the benefits and loads related to 'exported
the corresponding amounts are declared as material for energy electricity' and 'exported energy heat' resulting from the
recycling (MFR); energy recovery from plastic wastes in a municipal waste
- net amounts of a metal leaving the product system are incineration plant as modelled in Modules A3, A5 and C4.
5 Environmental Product Declaration - ARGE – The European Federation of Locks and Building Hardware Manufacturers - Hinges
5. LCA: Results
In Table 1 "Description of the system boundary", the declared modules are indicated with an "X"; all modules that are not declared
within the EPD but where additional data are available are indicated with "MND". Those data can also be used for building assessment
scenarios. The values are declared with three valid digits in exponential form.
The set of characterisation factors EF3.0 has been used for the life cycle assessment.
DESCRIPTION OF THE SYSTEM BOUNDARY (X = INCLUDED IN LCA; MND = MODULE OR INDICATOR NOT DECLARED; MNR
= MODULE NOT RELEVANT)
Benefits and
Construction loads beyond
Product stage Use stage End of life stage
process stage the system
boundaries
la ire wta am R y lp p u s tro p s n a rT g n iru tc a fu n a M tro p s nm ae o rh r
T
f t e h t o t ee tati gs y lb m e s s A e s U e c n a n e tn ia M ria p e R tn e m e c a lp e R tn e m h s ib ru fe R la n o ity ag rr ee pn Oe e s u la n o ita r re et pa Ow e s u n o itc u rts n eo Dc -n o itilo m e d tro p s n a rT g n is s ee tsc ao Wrp la s o p s iD e s u e R- y re v o c e R- g n ilc y c e R- la itn e to p
A1 A2 A3 A4 A5 B1 B2 B3 B4 B5 B6 B7 C1 C2 C3 C4 D
X X X X X MND MND MNR MNR MNR MND MND X X X X X
RESULTS OF THE LCA - ENVIRONMENTAL IMPACT according to EN 15804+A2: 1 kg of hinge
Parameter Unit A1-A3 A4 A5 C1 C2 C3 C4 D
GWP-total kg CO2 eq 7.37E+00 6.53E-01 2.33E-01 0 1.51E-02 3.16E-03 4.24E-03 -2.8E+00
GWP-fossil kg CO2 eq 7.56E+00 6.53E-01 2.34E-02 0 1.51E-02 3.15E-03 4.23E-03 -2.79E+00
GWP-biogenic kg CO2 eq -2.1E-01 0 2.1E-01 0 0 0 0 0
GWP-luluc kg CO2 eq 2.08E-02 2.61E-04 1.25E-06 0 6.02E-06 7.85E-06 3.36E-06 -8.82E-03
ODP kg CFC11 eq 4.16E-07 1.51E-07 6.93E-10 0 3.49E-09 1.6E-10 1.19E-09 -1.04E-07
AP mol H+ eq 7.73E-02 1.85E-03 1.72E-05 0 4.28E-05 1.62E-05 3.06E-05 -2.86E-02
EP-freshwater kg P eq 4.48E-04 4.65E-06 2.97E-08 0 1.07E-07 3.54E-07 6.54E-08 -1.74E-04
EP-marine kg N eq 9.46E-03 3.68E-04 6.12E-06 0 8.5E-06 2.08E-06 1.02E-05 -3.21E-03
EP-terrestrial mol N eq 1.06E-01 4.11E-03 6.61E-05 0 9.47E-05 2.4E-05 1.13E-04 -3.63E-02
kg NMVOC
POCP 3.09E-02 1.58E-03 1.85E-05 0 3.64E-05 6.57E-06 3.45E-05 -1.07E-02
eq
ADPE kg Sb eq 1.93E-03 2.31E-06 1.14E-08 0 5.34E-08 7.63E-09 1.4E-08 -9.5E-04
ADPF MJ 8.29E+01 9.89E+00 4.78E-02 0 2.28E-01 6.67E-02 9.04E-02 -2.88E+01
m3 world eq
WDP 1.96E+00 3.01E-02 3.01E-04 0 6.95E-04 7.45E-04 -1.18E-03 -7.76E-01
deprived
GWP = Global warming potential; ODP = Depletion potential of the stratospheric ozone layer; AP = Acidification potential of land and water; EP =
Eutrophication potential; POCP = Formation potential of tropospheric ozone photochemical oxidants; ADPE = Abiotic depletion potential for non-fossil
resources; ADPF = Abiotic depletion potential for fossil resources; WDP = Water (user) deprivation potential)
RESULTS OF THE LCA - INDICATORS TO DESCRIBE RESOURCE USE according to EN 15804+A2: 1 kg of hinge
Parameter Unit A1-A3 A4 A5 C1 C2 C3 C4 D
PERE MJ 9.62E+00 1.39E-01 -7.08E-01 0 3.21E-03 1.27E-02 2.35E-03 -3.71E+00
PERM MJ 1.79E+00 0 -2.19E-01 0 0 0 0 0
PERT MJ 1.14E+01 1.39E-01 -9.28E-01 0 3.21E-03 1.27E-02 2.35E-03 -3.71E+00
PENRE MJ 8.28E+01 9.9E+00 3.4E-01 0 2.28E-01 6.73E-02 9.04E-02 -2.89E+01
PENRM MJ 2.92E-01 0 -2.92E-01 0 0 0 0 0
PENRT MJ 8.3E+01 9.9E+00 4.78E-02 0 2.28E-01 6.73E-02 9.04E-02 -2.89E+01
SM kg 1.42E-01 0 0 0 0 0 0 0
RSF MJ 0 0 0 0 0 0 0 0
NRSF MJ 0 0 0 0 0 0 0 0
FW m3 7.09E-02 1.05E-03 5.2E-05 0 2.42E-05 4.3E-05 2.2E-04 -2.87E-02
PERE = Use of renewable primary energy excluding renewable primary energy resources used as raw materials; PERM = Use of renewable primary
energy resources used as raw materials; PERT = Total use of renewable primary energy resources; PENRE = Use of non-renewable primary energy
excluding non-renewable primary energy resources used as raw materials; PENRM = Use of non-renewable primary energy resources used as raw
materials; PENRT = Total use of non-renewable primary energy resources; SM = Use of secondary material; RSF = Use of renewable secondary fuels;
NRSF = Use of non-renewable secondary fuels; FW = Use of net fresh water
RESULTS OF THE LCA – WASTE CATEGORIES AND OUTPUT FLOWS according to EN 15804+A2:
1 kg of hinge
Parameter Unit A1-A3 A4 A5 C1 C2 C3 C4 D
HWD kg 4.8E-04 2.58E-05 2.15E-07 0 5.96E-07 2.37E-08 1.7E-07 -2.09E-05
NHWD kg 1.92E+00 5.21E-01 3.2E-03 0 1.2E-02 2.51E-04 3.81E-01 -3.81E-01
RWD kg 4.24E-04 1.43E-04 6.2E-07 0 3.3E-06 8.97E-07 1.17E-06 -1E-04
CRU kg 0 0 0 0 0 0 0 0
MFR kg 2E-01 0 9.35E-02 0 0 4.71E-01 0 0
MER kg 0 0 0 0 0 0 0 0
6 Environmental Product Declaration - ARGE – The European Federation of Locks and Building Hardware Manufacturers - Hinges
EEE MJ 0 0 3.71E-02 0 0 0 0 0
EET MJ 0 0 2.46E-01 0 0 0 0 0
HWD = Hazardous waste disposed; NHWD = Non-hazardous waste disposed; RWD = Radioactive waste disposed; CRU = Components for re-use;
MFR = Materials for recycling; MER = Materials for energy recovery; EEE = Exported electrical energy; EET = Exported thermal energy
RESULTS OF THE LCA – additional impact categories according to EN 15804+A2-optional:
1 kg of hinge
Parameter Unit A1-A3 A4 A5 C1 C2 C3 C4 D
Disease
PM 5.95E-07 5.24E-08 3.01E-10 0 1.21E-09 4.33E-11 9.52E-10 -2.05E-07
incidence
IR kBq U235 eq 1.98E-01 4.3E-02 1.89E-04 0 9.91E-04 6.08E-04 3.65E-04 -5.28E-02
ETP-fw CTUe 5.65E+02 7.77E+00 4.51E-02 0 1.79E-01 3.36E-02 1.25E+01 -2.32E+02
HTP-c CTUh 2.93E-08 2.5E-10 3.38E-12 0 5.76E-12 8.97E-13 9.21E-12 -1.14E-08
HTP-nc CTUh 1.26E-06 7.85E-09 1.37E-10 0 1.81E-10 2.91E-11 9.55E-11 -5.51E-07
SQP SQP 5.45E+01 6.9E+00 3.04E-02 0 1.59E-01 1.03E-02 1.56E-01 -1.43E+01
PM = Potential incidence of disease due to PM emissions; IR = Potential Human exposure efficiency relative to U235; ETP-fw = Potential comparative
Toxic Unit for ecosystems; HTP-c = Potential comparative Toxic Unit for humans (cancerogenic); HTP-nc = Potential comparative Toxic Unit for humans
(not cancerogenic); SQP = Potential soil quality index
Disclaimer 1 –
for the indicator 'Potential Human exposure efficiency relative to U235'. This impact category deals mainly with the eventual impact of
low-dose ionizing radiation on human health of the nuclear fuel cycle. It does not consider effects due to possible nuclear accidents,
occupational exposure or radioactive waste disposal in underground facilities. Potential ionizing radiation from the soil, radon and from
some construction materials is also not measured by this indicator.
Disclaimer 2 –
for the indicators 'abiotic depletion potential for non-fossil resources', 'abiotic depletion potential for fossil resources', 'water (user)
deprivation potential, deprivation-weighted water consumption', 'potential comparative toxic unit for ecosystems', 'potential comparative
toxic unit for humans – cancerogenic', 'Potential comparative toxic unit for humans - not cancerogenic', 'potential
soil quality index'. The results of this environmental impact indicator shall be used with care as the uncertainties on these results are
high as there is limited experience with the indicator.
6. LCA: Interpretation
Figure 1 illustrates the relative contributions of the different
modules along the life cycle of the declared products.
significant.
Figure 1: Environmental impacts of hinges along its life
cycle Benefits and burdens beyond the system boundary (module D)
are in the order of 15 % to 30 % of the impacts over the product
The largest part of environmental impacts is caused during life cycle (modules A1-A3) and relate basically to the recycling
production (modules A1-A3); comparably small impacts are of metals.
caused during the transport of the product to the construction
site (via the manufacturer of the product, which the hinges have A total of 6 typical products (based on sales figures) have been
been integrated into). evaluated and the worst-case results are used in section 5 of
this EPD. In chapter 2.5, the tabulated range of relative weight
All the other modules related to the product life cycle are not per material ensures that the variability of results stays within
7 Environmental Product Declaration - ARGE – The European Federation of Locks and Building Hardware Manufacturers - Hinges
+/- 40% of the declared values (assessed for the indicators GWP, PENRT, and non-hazardous waste).
7. Requisite evidence
No testing results are required by the PCR part B.
8. References
EAD 020001-01-0405, dated March 2017, Multi-axes
Product category rules of IBU concealed hinge assemblies.
IBU (2021) EN 13501-1
IBU (2021): General Instructions for the EPD Programme of the EN 13501-1:2018, Fire classification of construction products
Institut Bauen und Umwelt e.V. (General Instructions for the and building elements - Part 1: Classification using data from
IBU EPD Programme). Version 2.0, Institut Bauen und Umwelt, reaction to fire tests.
Berlin.
ISO 15686
IBU (2021) ISO 15686:1, -2, -7 and -8. Service life planning (various parts).
IBU (2021): PCR Part A: Calculation rules for the life cycle
assessment and requirements on the project report according Regulation No. 305/2011
to EN 15804+A2. Version 1.3., Institut Bauen und Umwelt, Regulation No. 305/2011 (Construction Products Regulation, or
Berlin. CPR) of the European Parliament and of the European Council
is a regulation of 9 March 2011 that lays down harmonised
IBU (2023) conditions for the marketing of construction products and
IBU (2023): PCR Part B: Requirements on the EPD for building replaces Construction Products Directive (89/106/EEC).
hardware products, Institut Bauen und Umwelt, Berlin.
ECHA candidate list
Standards and legal documents Candidate List of substances of very high concern for
Authorisation, published in accordance with Article 59(10) of the
EN 15804 REACH Regulation. European Chemicals Agency, Brussels.
EN 15804:2012+A2:2019+AC:2021, Sustainability of
construction works - Environmental product declarations - Core Ordinance on Biocide Products No. 528/2012
rules for the product category of construction products. REGULATION (EU) No 528/2012 OF THE EUROPEAN
PARLIAMENT AND OF THE COUNCIL of 22 May 2012
EN 17610 concerning the making available on the market and use of
EN 17610:2022, Building hardware - Environmental product biocidal products.
declarations - Product category rules complementary to EN
15804 for building hardware. European List of Waste
Commission Decision of 3 May 2000 replacing Decision
ISO 14025 94/3/EC establishing a list of wastes pursuant to Article 1(a) of
ISO 14025:2006-07, Environmental labels and declarations - Council Directive 75/442/EEC on waste and Council Decision
Type III Environmental declarations - Principles and 94/904/EC establishing a list of hazardous waste pursuant to
procedures. Article 1(4) of Council Directive 91/689/EEC on hazardous
waste (notified under document number C(2000) 1147).
ISO 14044
EN ISO 14044:2006-07, Environmental management - Life Additional references
cycle assessment - Requirements and guidance (ISO
14044:2006); German and English versions EN ISO BBSR 2017
14044:2006. BBSR (2017): Nutzungsdauer von Bauteilen in
Lebenszyklusanalysen nach Bewertungssystem Nachhaltiges
EN 1935 Bauen (BNB). Version vom 24.10.2017, Bundesinstitut für Bau-,
EN 1935:2002+AC:2003, Building hardware - Single-axis Stadt- und Raumforschung, Berlin.
hinges - Requirements and test methods.
ecoinvent v3.8
EAD 020001-01-0405 http://www.ecoinvent.org
8 Environmental Product Declaration - ARGE – The European Federation of Locks and Building Hardware Manufacturers - Hinges
Publisher
Institut Bauen und Umwelt e.V. +49 (0)30 3087748- 0
Hegelplatz 1 info@ibu-epd.com
10117 Berlin www.ibu-epd.com
Germany
Programme holder
Institut Bauen und Umwelt e.V. +49 (0)30 3087748- 0
Hegelplatz 1 info@ibu-epd.com
10117 Berlin www.ibu-epd.com
Germany
Author of the Life Cycle Assessment
Dr. Frank Werner - Umwelt & Entwicklung + 41 (0)44 241 39 06
Kammelenbergstrasse 30 frank@frankwerner.ch
9011 St. Gallen http://www.frankwerner.ch/
Switzerland
Owner of the Declaration
ARGE – The European Federation of Locks and +49 (0)2051 9506 15
Building Hardware Manufacturers mail@arge.org
Offerstraße 12 www.arge.org
42551 Velbert
Germany
9 Environmental Product Declaration - ARGE – The European Federation of Locks and Building Hardware Manufacturers - Hinges
