ENVIRONMENTAL PRODUCT DECLARATION
as per ISO 14025 and EN 15804+A2
Owner of the Declaration Sonae Arauco, S.A.
Publisher Institut Bauen und Umwelt e.V. (IBU)
Programme holder Institut Bauen und Umwelt e.V. (IBU)
Declaration number EPD-SON-20230515-IBA1-EN
Issue date 10.01.2024
Valid to 09.01.2029
Medium density fibreboard (MDF), coated
Sonae Arauco, S.A.
www.ibu-epd.com | https://epd-online.com
1. General Information
Sonae Arauco, S.A. Medium density fibreboard (MDF), coated
Programme holder Owner of the declaration
IBU – Institut Bauen und Umwelt e.V. Sonae Arauco, S.A.
Hegelplatz 1 Calle Ulises 26­18
10117 Berlin 28043 Madrid
Germany Spain
Declaration number Declared product / declared unit
EPD­SON­20230515­IBA1­EN Medium density fibreboard, coated with melamine­impregnated paper, per
m2
This declaration is based on the product category rules: Scope:
Wood­based panels, 01.08.2021 This document refers to MDF manufactured in the following plants of the
(PCR checked and approved by the SVR) Sonae Arauco Group:
• Sonae Arauco Beeskow GmbH, Radinkendorfer Strasse 71,
15848 Beeskow, Germany
Issue date
• Sonae Arauco Deutschland GmbH ­ Nettgau Plant, Strohmweg
10.01.2024 1, 38489 Nettgau, Germany
• Sonae Arauco Portugal S.A., Estrada Nacional 17, nº 59 e 61,
3400­691 S.Paio de Gramaças (Oliveira do Hospital), Portugal
Valid to • Sonae Arauco South Africa (Pty) Ltd, Heidelberg Road, Rocky
Drift, White River, Republic of South Africa
09.01.2029
• Sonae Arauco España­Soluciones de Madera, S.L., Carretera
Córdoba­Valencia Km 126, Estación Linares­Baeza, 23490
Linares (Jaén), Spain
The production volume of these plants covers 100 % of the total production
of coated MDF by Sonae Arauco group.
The owner of the declaration shall be liable for the underlying information
and evidence; the IBU shall not be liable with respect to manufacturer
information, life cycle assessment data and evidences.
The EPD was created according to the specifications of EN 15804+A2. In
the following, the standard will be simplified as EN 15804.
Dipl.­Ing. Hans Peters Verification
(Chairman of Institut Bauen und Umwelt e.V.)
The standard EN 15804 serves as the core PCR
Independent verification of the declaration and data according to ISO
14025:2011
internally X externally
Florian Pronold Mr Olivier Muller,
(Managing Director Institut Bauen und Umwelt e.V.) (Independent verifier)
1 Environmental Product Declaration ­ Sonae Arauco, S.A. ­ Medium density fibreboard (MDF), coated
2. Product
available at:
2.1 Product description/Product definition www.sonaearauco.com
Medium density fibreboard (MDF) is a panel­shaped wood­
based material in accordance with EN 316 that is manufactured Reference technical properties for coated MDF according to EN
in a dry process by means of compression under heat of wood 14322:2021 are presented in the table below as reference
fibres with adhesive. Coated MDF boards can be profiled. MDF values (special boards, as well as customized products can
can be coated with melamine facing according to EN 14322. have different values).
Due to their various densities and adhesive systems, they can
display a variety of material properties and qualities like
moisture resistance, fire retardant, load­bearing or others.
For the placing on the market of the product in the European
Union/European Free Trade Association (EU/EFTA) (with the
exception of Switzerland), Regulation (EU) No. 305/2011 (CPR)
applies. When applicable, the product needs a declaration of
performance taking into consideration EN 13986:2004+A1:2015
Wood-based panels for use in construction - Characteristics,
evaluation of conformity and marking and the CE­marking.
For the application and use the respective national provisions
apply.
2.4 Delivery status
2.2 Application
MDF ranging in thicknesses from 3 to 40 mm can be purchased
The area of application for uncoated MDF primarily involves
as coated boards. The boards are offered in standard formats.
decorative interior furnishings and furniture construction but
Fixed formats are also available, and selected formats are
also interior construction such as trade fair stands and shop
offered with a tongue and groove profile.
design.
When painted or coated, MDF can also be found in kitchens,
The following values indicate typical minimum and maximum
offices, bedrooms and living rooms.
dimensions for the boards supplied worldwide. Some of the
Apart from an extensive basic range, special MDF variants are
combinations for sizes may not be available in all markets.
also available, e.g. fire­retardant MDF as well as MDF with
increased resistance to moisture.
Thickness: 3 – 40 mm
2.3 Technical Data Width: 650 – 2465 mm
Due to the large variability of product properties and quality Length: 1740 – 5600 mm
grades, the table below only shows the range of technical
characteristics for standard boards. For updated information on available dimensions, please refer
to:
Special boards as well as customized products have different
technical characteristics from the ones shown, that are referring www.sonaearauco.com
to the core board used for surfacing.
2.5 Base materials/Ancillary materials
Name Value Unit
Coated MDF bonded with urea­formaldehyde/melamine­urea­
Gross density according to EN 323 680 ­ 860 kg/m3 formaldehyde (UF/MUF) consist of (dimensions as % by mass):
Bending strength (longitudinal) according to
17 ­ 23 N/mm2 • Wood chips: approx. 80 %
EN 310
• Water: 4 – 11 %
E­module (longitudinal) according to EN 1900 ­ • UF glue / MUF glue (urea resin, melamine urea resin): 9
N/mm2
310 2700 – 25 %
Material dampness at delivery according to • Paraffin wax emulsion, 0.5 – 3 %
5 ­ 9 %
EN 322 • Impregnated paper: 0.5 – 4 %
Material dampness at delivery ­ % Coated MDF bonded with polymeric diphenylmethane
diiscocyanate (PMDI) consist of (dimensions as % by mass):
Tensile strength rectangular according to
0.5 ­ 0.65 N/mm2
EN 319 • Wood chips: approx. 90%
• Water: 5 – 9%
Thickness swelling according to EN 317 8 ­ 45 %
• PMDI glue (polymer 4.4' diphenyl methane
Performance data of the product in accordance with the diisocyanate): approx. 3.5 %
declaration of performance with respect to its essential • Paraffin wax emulsion: 0.5 – 3%
characteristics according to: • Impregnated paper: 0.5 – 4 %
EN 316, Wood fibre boards Wood from indigenous, largely regional forest plantations is
EN 622-1, Fibreboards used for manufacturing MDF. This wood is typically procured
EN 622-5, Fibreboards from forests within an averae radius of 250 km of the plants'
EN 13986 Wood-based panels for use in construction locations.
ISO 16895-1, Wood-based panels Furthermore, sawmill residues are also used as raw materials
ISO 16895-2, Wood-based panels in the production of MDF.
Declaration of Performance (DoP) The entire range can be made available on request as FSC®
certified or PEFC (program for the endorsement of forest
For more details on technical information, please see the
certification) certified products.
respective products' Declaration of Performance (DoP)
Additionally, tne complete range includes CE­marked products.
2 Environmental Product Declaration ­ Sonae Arauco, S.A. ­ Medium density fibreboard (MDF), coated
7. Scattering the glued fibre on a forming belt
This product contains substances listed in the ECHA candidate 8. Pressing the fibre mat in a continuous hot press under high
list (date: 08.06.2021) exceeding 0.1 percentage by mass: pressure
· no 9. Cutting the continuous mat into raw board formats
10. Cooling the raw boards in star coolers
This product contains other carcinogenic, mutagenic, reprotoxic 11. Stacking
(CMR) substances in categories 1A or 1B which are not on the 12. Sanding the top or underside after the air­conditioning
ECHA candidate list, exceeding 0.1 percentage by mass: phase
· no 13. Surfacing with impregnated paper in a short cycle press
Biocide products were added to this construction product or it Finally, the panels are coated with melamine­impregnated
has been treated with biocide products (this then concerns a paper in a short­cycle press.
treated product as defined by the (EU) Ordinance on Biocide
Products No. 528/2012: All leftovers incurred during board manufacture are redirected
· no to be used as fuel to supply the energy needs of the
manufacturing process on site.
2.6 Manufacture
The manufacturing comprises the following steps: A process diagram is presented below.
The production sites are certified according to the following
1. Debarking the logs standards:
2. Chipping the wood to chips of approx. 3 x 3 cm in size
• ISO 9001
3. Boiling the chips
• ISO 45001
4. Defibring in the refiner
• EN ISO 50001 (European sites).
5. Glueing the fibres with resin
6. Drying the fibres to a residual moisture content
Emissions into air: Waste air generated during production is
2.7 Environment and health during manufacturing cleaned in accordance with regulatory requirements. Emissions
Health protection: Due to the manufacturing conditions, no have to comply with the values specified by the operation
special health protection measures over and beyond the licenses of the different sites, specified according to national
regulatory guidelines are required. The reference occupational laws.
exposure limit values are complied with.
Emissions into water/soil: No normal process contamination
3 Environmental Product Declaration ­ Sonae Arauco, S.A. ­ Medium density fibreboard (MDF), coated
of water or soil exists. Waste water generated in the process is
treated onsite and/or directed into the municipal sewage 2.12 Reference service life
system following pre­treatment. Sludges generated within the Due to the wide range of applications of Sonae Arauco coated
water treatment can be used in agriculture as a fertiliser. MDF, no reference service life is declared.
2.13 Extraordinary effects
Noise: Noise surveys are required and are performed for each
site according to respective national regulations. Noise­ Fire
intensive plant areas such as chipping are encapsulated or Fire retardant classification is done according to EN 13986. Fire
protected appropriately by structural measures. retardant classes are defined in accordance with EN 13501-1.
Whenever necessary (close to non­encapsulated areas), the
use of ear protection is required (PPE, Personal Protective The fire classification of coated MDF with a raw density of ≥
Equipment) within Sonae Arauco sites, as an additional safety 600 kg/m³ and a thickness ≥ 9 mm is D­s2, d0. The boards with
measure. lower density or thickness are in class E.
The production sites are all ISO 14001 certified. Fire retardant boards are classified as B­s1, d0 and B­s2, d0.
Fire safety (for standard MDF boards)
2.8 Product processing/Installation
Name Value
Sonae Arauco coated MDF can be sawn, milled, sanded and
Building material class D/E
drilled using standard machinery or (electric) power tools.
Carbide­tipped tools should be given preference, especially on Smoke gas development S2
circular saws. Respiratory protection should be worn when Burning droplets d0
using hand­held equipment without suction devices.
Water
Please refer to the respective devices' datasheets for further
No ingredients are washed out which could be hazardous to
processing recommendations.
water. Coated MDF is not resistant to permanent exposure to
2.9 Packaging water.
Sonae Arauco coated MDF is supplied on squared timber
Mechanical destruction
bound by plastic or metal bands and covered with corrugated
Mechanical destruction of coated MDF boards can result in
cardboard and, on the bottom, with a cover board.
sharp edges on the broken panel edges (risk of injury).
MDF and steel or PET packing bands for transport packaging
2.14 Re-use phase
can be sorted and directed to the recycling circuits. If re­use or
Recycling: Sonae Arauco coated MDF from construction can
recycling is impractical, the packaging should not be landfilled,
be collected separately and utilised in the manufacture of MDF
but rather directed towards energy recovery.
or other types of wood­based boards. This is based on the
condition that the wooden boards are not fully glued.
Packaging disposal information is available at:
www.sonaearauco.com
Energy recovery: Due to the high heating value of approx.
2.10 Condition of use 16.2 MJ/kg at 20 % moisture content assumed for post­
consumer boards, coated MDF can be used for energy
The components making up coated MDF correspond with the
recovery and the generation of heat and electricity (e.g. in CHP
base material compositions as outlined in Clause 2.6. During
plants), following the cascading principle for wood.
hot pressing, the binding agent is linked irreversibly by means
of poly­condensation and firmly bonded with the wood. The
2.15 Disposal
binding agents are chemically and stably bound to the wood.
Sonae Arauco coated MDF leftovers and residual materials
incurred as a result of demolition measures on the building sites
VOC emissions: Sonae Arauco coated MDF is labelled as
should be primarily directed towards material recycling. If this is
class A+ according to the French regulation on the labelling of
not possible, they must be directed toward energy recovery
emissions of volatile pollutants from construction and
instead of landfilling.
decoration products (with reference to the wall scenario, as a
worst case).
Waste code according to the European List of Waste: 17 02 01
Sonae Arauco MDF, coated with melamine impregnated paper 2.16 Further information
at an average area weight of 13.3 kg/m2 stores 19.5 kg CO 2 Further information such as technical datasheets, etc. can be
equivalent over its service life. downloaded under:
2.11 Environment and health during use
www.sonaearauco.com
Environmental protection: According to current information,
water, air and soil are not exposed to any dangers when the
respective products outlined above are used as designated.
Health protection: According to current information, no
damage to or impairment of health can be anticipated when
MDF is used as designated.
With the exception of low volumes of formaldehyde for
UF/MUF­bonded MDF, VOC emissions from products are
negligible, and are natural wood ingredients.
4 Environmental Product Declaration ­ Sonae Arauco, S.A. ­ Medium density fibreboard (MDF), coated
3. LCA: Calculation rules
Therefore, module D covers the avoided burdens from recycling
3.1 Declared Unit and from energy recovered from the waste treatment in module
The declared unit for the LCA is 1 m2 of average Sonae Aracuo A5 as well as the transport of the obsolete boards to a biomass
medium density fibreboard (MDF), coated with melamine combustion plant, the combustion process itself and the loads
impregnated paper. and benefits of the substitution of fossil fuels and/or electricity.
Substitution effects in module D are always calculated for the
Information on the declared unit
net amount of secondary material or secondary fuel of the
Name Value Unit
product system in line with EN 16485.
Declared unit 1 m2
3.3 Estimates and assumptions
Grammage 13.3 kg/m2
For the quantification of the net flows of recycled wood (input of
Layer thickness 0.0169 m
post­consumer wood used as a fuel minus post­consumer
The weighted average was calculated based on production wood exiting the product system into module D for energy
volumes from the plants in all countries where Sonae Arauco recovery), it was assumed that all inputs of post­consumer
was operating in 2021 (some plants: 2020). wood are used as a fuel; inputs of post­consumer wood beyond
the need of wood fuel used in production was considered to be
3.2 System boundary
used as a recycled material input.
Type of the EPD: cradle­to­gate with modules C1 to C4 and Beyond that, no relevant estimates or assumptions had to be
module D (A1­A3, C and D) made beyond the information provided in this EPD.
Modules A1 – A3 of the production stage cover the 3.4 Cut-off criteria
manufacturing of the products, including raw material extraction All data were taken into account that resulted from the data
and processing, energy generation, the production of ancillary collection procedure in the plants, e.g. related to fuels, raw
products and packaging materials, transport, as well as all material input, use of ancillary materials, waste flows,
waste treatment processes. Eventual benefits of recycling or emissions into the air, water use, waste water, transport means
energy recovery are neglected. and transport distances, etc..
The resource aspects of wood were inventoried via material Expenses for the general management, research &
inherent properties such as resource extraction of CO from the development, administration and marketing – if known – were
2
atmosphere and the lower heating value as the use of not taken into account.
renewable energy. Material inherent properties are subject to The production of eventual packaging of ancillary material or
co­product allocation as ruled in EN 15804. other inputs used during production (and some of the reported
wastes) were generally neglected; in most cases reusable bins
Module A4 covers the transport of the product from the or containers are used. In addition, the amounts of reported
production site to the construction site by a lorry over a default (unspecific) wastes are so small that their production can be
distance of 460 km. considered not relevant for the life cycle assessment. Additional
plant specific information can be found in the respective
Module A5 covers the transport of the packaging material from chapters for each plant.
the construction site and its disposal. Default end­of­waste Beyond that some plants reported ancillary materials that were
states for the packaging materials from the packed products at cut off due to very small amounts and as inputs not directly
the construction site are defined in analogy for wastes related to production processes but to the maintenance of
occurring in modules A1­A3. Eventual further inputs for the infrastructure, e.g. acetylene and oxygen for soldering, etc.
installation of the products are not considered due to the broad With this approach mass and energy flows below 1 percent of
applicability of the assessed products. total mass and energy flows caused by the declared products
The substituted primary material from the net amount of were included in the assessment.
recycled material and from recovered energy exported from the Beyond that, no material or energy flows were neglected that
product system in Module A5 is declared in Module D. would have been known by the persons responsible for the
project and that could have been expected to contribute
Module C1 manual deconstruction is assumed. The declared significantly to the environmental indicators declared. It can
values are thus 0. thus be assumed that the total contribution of the neglected
processes is not higher than 5 % of the declared impact
Module C2 includes the transport of the de­constructed product categories.
to a recycling centre by over 50 km.
3.5 Background data
Module C3 covers the preparation of the post­consumer board Datasets from ecoinvent 3.8 (cut­off by classification) were
to become a secondary fuel; the end­of­waste status for used as background data exclusively. Therefore, the latest
recycled wood­based boards is defined as the point where they update of the background data took place in 2021.
have been sorted and chipped, ready to be used as secondary
3.6 Data quality
fuels.
The requirements on the data quality and the background data
In line with EN 16485, the export of the biogenic carbon stored
correspond to the provisions in EN 15804:
in the board, expressed in CO ­equivalent is also reported in
2
module C3. • Data are as current as possible. Datasets used for
Module C4 is not relevant for the assumed end­of­life scenario. calculations were updated within the last 10 years for
The declared values are thus 0. generic data and within the last 5 years for producer­
specific data;
Module D compiles all the benefits and burdens associated with • Datasets are based on 1­year averaged data as a
the secondary fuels, secondary materials and exported energy general rule;
leaving the production system in the modules A5 and C3.
5 Environmental Product Declaration ­ Sonae Arauco, S.A. ­ Medium density fibreboard (MDF), coated
• The time period over which inputs to and outputs from process.
the system are accounted for is 100 years from the year In the case of sites where several products were produced and
for which the data set is deemed representative; no product­specific information was available, all inputs and
• The technological coverage reflects the physical reality outputs related to production processes were attributed based
of the declared products; on a total mass of production; packaging material was
• The background datasets comply with the quality attributed based on a total volume of the production. Inputs and
guidelines of ecoinvent v.3; deviations from the outputs for coating processes that could not be separated from
methodological prescriptions of EN 15804 cannot be the data on plant level were conservatively attributed to the
excluded but are considered not significant in the production of MDF.
context of this EPD. Post­consumer secondary wood is used as an input to produce
particleboard; for this input as well as for the end­of­life
3.7 Period under review scenario, the end­of­waste status was defined after the sorting
The company data gathered for this EPD represents the year and chipping of the wood­based board in line with EN 16485
2020/21. (see also clause 3.2). In analogy, MDF leaving the product
system at the end­of­life is considered a secondary fuel; its
3.8 Geographic Representativeness
combustion and the benefits of energy recovery are declared in
Land or region, in which the declared product system is module D.
manufactured, used or handled at the end of the product´s Waste packaging in module A5 was considered not to reach the
lifespan: Europe end­of­waste state as a fuel. Its incineration is reported in A5,
the benefits of energy recovery in module D. The benefits of the
recycling of minor amounts of packaging materials are
3.9 Allocation
disregarded.
The inventories for the wood inputs were taken from ecoinvent
No co­product allocation was made in the modelling of the
v.8. In ecoinvent, the forestry processes are modelled on a
foreground data of the life cycle assessment underlying this
mass­basis and sawmilling processes are allocated based on
EPD.
revenues of the different co­products of a joint co­production
process. 3.10 Comparability
Waste generated by edge­trimming and cut­size saws is used
Basically, a comparison or an evaluation of EPD data is only
internally for energy generation. Some plants sell minor
possible if all the data sets to be compared were created
quantities of bark or electricity from co­generation. No impacts
according to EN 15804 and the building context, respectively
are allocated to these outputs.
the product­specific characteristics of performance, are taken
Biogenic carbon (content) is modelled manually thus reflecst
into account. ecoinvent v3.8 (cut­off by classification) has been
the real physical flows; this is not the case for primary energy,
used as the background database
implying that the content of primary energy in products and
packaging is allocated as the main inputs/outputs of a unit
4. LCA: Scenarios and additional technical information
waste input; 92 % of the recovered energy is heat, 8 % is
Characteristic product properties of biogenic carbon electricity (according to specifications of MWI plants in
Note: 1 kg of biogenic carbon is equivalent to 44/12 kg of CO 2. ecoinvent 3.8).
Information on describing the biogenic Carbon Content at
Deconstruction (C1)
factury gate
Manual deconstruction is assumed. The declared values are
Name Value Unit
thus 0.
kg
Biogenic carbon content in product 6.42
C Transport to waste treatment (C2)
Biogenic carbon content in accompanying kg This module includes the transport of the de­constructed
0.00245
packaging C product to a recycling centre by a lorry (15 % emissions class
EURO 5; 85 % emissions class EURO 6) by over 50 km.
The following technical information is a basis for the declared
Waste treatment (C3)
modules or can be used for developing specific scenarios in the
15,2 kg of coated MDF are chipped and exported from the
context of a building assessment if modules are not declared
product life cycle into module D, assuming a moisture content
(MND).
of 20 % and a lower heating value of 16,2 MJ/kg. The biogenic
carbon stored in the product and the content of primary energy
Transport to the construction site (A4)
are exported from the product system as material inherent
The product is transported from the production site to the
properties.
construction site by a lorry (15 % emissions class EURO 5; 85
% emissions class EURO 6) over a default distance of 460 km.
Disposal (C4)
This module is not relevant for the assumed end­of­life
Installation into the building (A5)
scenario. The declared values are thus 0.
Eventual further inputs for the installation of the products are
not considered due to the broad applicability of the assessed
Reuse, recycling, recovery potential (D)
products.
According to default assumptions in other IBU EPDs, post­
An average transport distance of 30 km was assumed for
consumer wood is used as a secondary fuel for energy
packaging waste from the construction site to the recycling
recovery in a biomass combustion plant with an overall energy
plant or to the municipal waste incineration plant. The municipal
efficiency of 93 % related to the lower heating value of the fuel
waste incineration plant is assumed to have an overall energy
input; 91 % of the recovered energy is heat, 9 % is electricity.
efficiency of 53 % related to the lower heating value of the
6 Environmental Product Declaration ­ Sonae Arauco, S.A. ­ Medium density fibreboard (MDF), coated
5. LCA: Results
DESCRIPTION OF THE SYSTEM BOUNDARY (X = INCLUDED IN LCA; MND = MODULE OR INDICATOR NOT DECLARED; MNR
= MODULE NOT RELEVANT)
Benefits and
Construction loads beyond
Product stage Use stage End of life stage
process stage the system
boundaries
la ire ta m w a Ry lp p u s tro p s n a rT g n iru tc a fu n a M e h t m o rf tro p s n a rTe tis e h t o t e ta g y lb m e s s A e s U e c n a n e tn ia M ria p e R tn e m e c a lp e R tn e m h s ib ru fe R y g re n e la n o ita re p Oe s u re ta w la n o ita re p Oe s u n o itc u rts n o c ­e Dn o itilo m e d tro p s n a rT g n is s e c o rp e ts a W la s o p s iD ­e s u e R­y re v o c e R­g n ilc y c e Rla itn e to p
A1 A2 A3 A4 A5 B1 B2 B3 B4 B5 B6 B7 C1 C2 C3 C4 D
X X X X X MND MND MNR MNR MNR MND MND X X X X X
RESULTS OF THE LCA - ENVIRONMENTAL IMPACT according to EN 15804+A2: Medium density fibreboard (MDF), coated
with melamine-impregnated paper, per m²
Parameter Unit A1-A3 A4 A5 C1 C2 C3 C4 D
GWP­total kg CO 2 eq ­4.73E+00 1E+00 1.66E+00 0 1.42E­01 1.66E+01 0 ­9.74E+00
GWP­fossil kg CO 2 eq 1.19E+01 1E+00 1.46E+00 0 1.42E­01 1.23E­01 0 ­9.73E+00
GWP­biogenic kg CO 2 eq ­1.67E+01 0 1.98E­01 0 0 1.65E+01 0 0
GWP­luluc kg CO 2 eq 2.95E­02 3.99E­04 4.93E­05 0 6.72E­05 2.83E­04 0 ­5.14E­03
ODP kg CFC11 eq 1.4E­06 2.32E­07 1.21E­07 0 3.2E­08 6.2E­09 0 ­1.88E­06
AP mol H+ eq 7.85E­02 3.03E­03 3.39E­03 0 4.27E­04 6.59E­04 0 ­1.47E­02
EP­freshwater kg P eq 4.94E­04 7.11E­06 9.61E­07 0 1.16E­06 1.28E­05 0 ­2.28E­04
EP­marine kg N eq 1.41E­02 6.63E­04 1.45E­03 0 8.94E­05 8.94E­05 0 ­1.6E­03
EP­terrestrial mol N eq 1.88E­01 7.37E­03 1.59E­02 0 9.97E­04 1.02E­03 0 ­1.77E­02
kg NMVOC
POCP 7.27E­02 2.67E­03 5.59E­03 0 3.62E­04 2.88E­04 0 ­7.63E­03
eq
ADPE kg Sb eq 1.24E­04 3.54E­06 4.75E­07 0 6.5E­07 3.4E­07 0 ­5.42E­06
ADPF MJ 2.09E+02 1.52E+01 7.37E+00 0 2.13E+00 2.57E+00 0 ­2.47E+02
m3 world eq
WDP 1.31E+01 4.6E­02 3.81E­03 0 7.05E­03 2.99E­02 0 ­2.93E­01
deprived
GWP = Global warming potential; ODP = Depletion potential of the stratospheric ozone layer; AP = Acidification potential of land and water; EP =
Eutrophication potential; POCP = Formation potential of tropospheric ozone photochemical oxidants; ADPE = Abiotic depletion potential for non­fossil
resources; ADPF = Abiotic depletion potential for fossil resources; WDP = Water (user) deprivation potential)
RESULTS OF THE LCA - INDICATORS TO DESCRIBE RESOURCE USE according to EN 15804+A2: Medium density fibreboard
(MDF), coated with melamine-impregnated paper, per m²
Parameter Unit A1-A3 A4 A5 C1 C2 C3 C4 D
PERE MJ 5.7E+01 2.13E­01 1.36E­01 0 3.54E­02 4.47E­01 0 ­8.23E+00
PERM MJ 2.03E+02 0 ­9.75E­02 0 0 ­2.03E+02 0 0
PERT MJ 2.6E+02 2.13E­01 3.89E­02 0 3.54E­02 ­2.03E+02 0 ­8.23E+00
PENRE MJ 1.68E+02 1.52E+01 7.38E+00 0 2.13E+00 2.59E+00 0 ­2.47E+02
PENRM MJ 4.04E+01 0 ­4.83E­03 0 0 ­4.04E+01 0 0
PENRT MJ 2.09E+02 1.52E+01 7.37E+00 0 2.13E+00 ­3.78E+01 0 ­2.47E+02
SM kg 0 0 0 0 0 0 0 0
RSF MJ 1.81E+01 0 0 0 0 0 0 1.81E+02
NRSF MJ 0 0 0 0 0 0 0 7.43E+00
FW m3 3.2E­01 1.61E­03 2.91E­04 0 2.91E­04 1.57E­03 0 ­2E­02
PERE = Use of renewable primary energy excluding renewable primary energy resources used as raw materials; PERM = Use of renewable primary
energy resources used as raw materials; PERT = Total use of renewable primary energy resources; PENRE = Use of non­renewable primary energy
excluding non­renewable primary energy resources used as raw materials; PENRM = Use of non­renewable primary energy resources used as raw
materials; PENRT = Total use of non­renewable primary energy resources; SM = Use of secondary material; RSF = Use of renewable secondary fuels;
NRSF = Use of non­renewable secondary fuels; FW = Use of net fresh water
RESULTS OF THE LCA – WASTE CATEGORIES AND OUTPUT FLOWS according to EN 15804+A2:
Medium density fibreboard (MDF), coated with melamine-impregnated paper, per m²
Parameter Unit A1-A3 A4 A5 C1 C2 C3 C4 D
HWD kg 2.82E­04 3.96E­05 2.5E­06 0 5.7E­06 1.2E­06 0 ­2.69E­04
NHWD kg 2.33E+00 7.96E­01 3.93E­02 0 9.11E­02 1.7E­02 0 2.54E­01
RWD kg 9.46E­04 2.19E­04 1.12E­04 0 3.05E­05 3.37E­05 0 ­7.8E­04
CRU kg 0 0 0 0 0 0 0 0
MFR kg 5.1E­02 0 2.54E­04 0 0 0 0 0
MER kg 0 0 0 0 0 1.52E+01 0 0
EEE MJ 8.06E­01 0 3.47E­03 0 0 0 0 0
EET MJ 8.16E+00 0 3.99E­02 0 0 0 0 0
7 Environmental Product Declaration ­ Sonae Arauco, S.A. ­ Medium density fibreboard (MDF), coated
HWD = Hazardous waste disposed; NHWD = Non­hazardous waste disposed; RWD = Radioactive waste disposed; CRU = Components for re­use;
MFR = Materials for recycling; MER = Materials for energy recovery; EEE = Exported electrical energy; EET = Exported thermal energy
RESULTS OF THE LCA – additional impact categories according to EN 15804+A2-optional:
Medium density fibreboard (MDF), coated with melamine-impregnated paper, per m²
Parameter Unit A1-A3 A4 A5 C1 C2 C3 C4 D
Disease
PM 6.51E­07 6.41E­08 7.6E­08 0 7.82E­09 2.01E­09 0 ­1.3E­08
incidence
IR kBq U235 eq 4.4E­01 6.58E­02 3.19E­02 0 9.25E­03 2.27E­02 0 ­4.46E­01
ETP­fw CTUe 3.16E+02 1.19E+01 4.01E+00 0 1.74E+00 1.46E+00 0 ­1.88E+01
HTP­c CTUh 8.14E­08 3.83E­10 7.15E­11 0 6.28E­11 6.92E­11 0 2.16E­09
HTP­nc CTUh 1.81E­07 1.21E­08 2.85E­09 0 1.69E­09 1.26E­09 0 ­8.54E­10
SQP SQP 1.45E+03 1.05E+01 1.32E+00 0 1.26E+00 3.96E­01 0 ­6.87E+00
PM = Potential incidence of disease due to PM emissions; IR = Potential Human exposure efficiency relative to U235; ETP­fw = Potential comparative
Toxic Unit for ecosystems; HTP­c = Potential comparative Toxic Unit for humans (cancerogenic); HTP­nc = Potential comparative Toxic Unit for humans
(not cancerogenic); SQP = Potential soil quality index
Disclaimer 1 – for the indicator “Potential Human exposure efficiency relative to U235”. This impact category deals mainly with the
eventual impact of low­dose ionizing radiation on human health of the nuclear fuel cycle. It does not consider effects due to possible
nuclear accidents, occupational exposure or radioactive waste disposal in underground facilities. Potential ionizing radiation from the
soil, radon and from some construction materials is also not measured by this indicator.
Disclaimer 2 – for the indicators “abiotic depletion potential for non­fossil resources”, “abiotic depletion potential for fossil resources”,
“water (user) deprivation potential, deprivation­weighted water consumption”, “potential comparative toxic unit for ecosystems”,
“potential comparative toxic unit for humans – cancerogenic”, “Potential comparative toxic unit for humans ­ not cancerogenic”,
“potential soil quality index”. The results of this environmental impact indicator shall be used with care as the uncertainties on these
results are high as there is limited experience with the indicator.
6. LCA: Interpretation
Figure 1 illustrates the contribution of each life cycle stage to fibreboard (MDF).
the overall indicator results of the impact assessment (impact
from module A1­C4 = 100 %) for coated medium denstity
medium density fibreboard (MDF) is dominated by the
Figure 1: Environmental impacts of medium density production phase (modules A1­A3). Minor contributions stem
fibreboard (MDF) coated with melamine-impregnated paper from transport to the construction site whereas the contributions
along its life cycle (impacts from production modules A1- from other modules of the life cycle are negligible.­Loads and
C4 = 100 %) benefits beyond the life cycle (module D) are negative
(benefits > loads) whereas major contributions occur for the
Figure 1 illustrates that the environmental profile of coated ODP, the GWP­fossil and for the ADPF; these benefits basically
8 Environmental Product Declaration ­ Sonae Arauco, S.A. ­ Medium density fibreboard (MDF), coated
stem from the use of the medium density fibreboard (MDF) as
secondary fuel and its related substitution of natural gas and
electricity from the grid from the recovered energy.
Figure 2 illustrates that the biogenic carbon stored in the
medium density fibreboard (MDF) coated with melamine im
pregnated paper, expressed as CO ­equivalent, is higher than
2
the CO emissions from fossil sources, leading to a negative
2
GWP for the production module A1­A3. The potential
substitution effect in mod­ule D offsets the GHG emissions
during the production phase (module A1­A3).
Figure 2: Greenhouse Gas balance of medium density
fibreboard (MDF) coated with melamine-impregnated paper
The GWP is dominated by CO emissions and removals.
2
7. Requisite evidence
7.3 VOC emissions
7.1 Formaldehyde
For UF/MUF bonded boards: Measuring agency: Fraunhofer Institut für Holzforschung
Wilhem­Klauditz­Institut WKI
Measuring agency: Aidimme Technology Institute, Valencia, Test report, date: MAIC­2019­4891, issued on the 17.12.2019
Spain Result: AgBB/ABG requirements were complied with.
Test report, date: no. 221.I.2303.329.EN.01 issued on the
AgBB overview of results (28 days [µg/m³])
15.03.2023
Name Value Unit
Result: Formaldehyde emission testing according to ASTM
D6007-14 was performed using EN 717 for formaldehyde TVOC (C6 ­ C16) 41 μg/m3
concentration determination. A value of 0,074 ppm was Sum SVOC (C16 ­ C22) ­ μg/m3
determined.
R (dimensionless) 0.285 ­
VOC without NIK ­ μg/m3
Measuring agency: MPA Eberswalde, Materialprüfanstalt
Brandenburg GmbH, Germany Carcinogenic Substances < 1 μg/m3
Test report, date: No. 31/23/4267/01/QT issued on the
17.04.2023 AgBB overview of results (3 days [µg/m³])
Result: Determination of formaldehyde release of wood based Name Value Unit
panels according to: TVOC (C6 ­ C16) 45 μg/m3
CARB final regulation order of "Airborne toxic control measure
Sum SVOC (C16 ­ C22) 0 μg/m3
to reduce Formaldehyde emission from composite Wood
products" and EPA TSCA Title VI 40 CFR Part 770. R (dimensionless) 0.288 ­
Formaldehyde analysis by photometry by acetyl/acetone VOC without NIK 0 μg/m3
method according to EN 717­1. Carcinogenic Substances 0 μg/m3
Requirement of CARB and EPA TSCA VI was met.
.
7.4 PCP/Lindane
7.2 Checking for the pretreatment of the substances used
Measuring agency: MPA Eberswalde, Materialprüfanstalt
No post­consumer wood is used in the production of Sonae Brandenburg GmbH, Germany
Arauco MDF. Test report, date: 31/21/2228/01PL issued at 15.04.2021
Result: Neither PCP nor Lindan content were detected. This
means that neither PCP nor Lindan were present in a quantity
. above the the method limit of quantification.
9 Environmental Product Declaration ­ Sonae Arauco, S.A. ­ Medium density fibreboard (MDF), coated
8. References
Product category rules of IBU
EN 12524
IBU (2021) EN 12524:2000, Building materials and products –
IBU (2021): General Instructions for the EPD Programme of the Hygrothermal properties – Tabulated design values.
Institut Bauen und Umwelt e.V. (General Instructions for the
IBU EPD Programme). Version 2.0, Institut Bauen und Umwelt, EN 13501
Berlin. EN 13501­1:2019, Fire classification of construction products
and building elements – Classification using test data from
IBU (2021) reaction to fire tests.
IBU (2021): PCR Part A: Calculation rules for the life cycle
assessment and requirements for the project report according EN 13986
to EN 15804+A2:2019. Version 1.3, Institut Bauen und Umwelt, EN 13986:2015, Wood­based panels for use in construction –
Berlin. Characteristics, evaluation of conformity and marking.
IBU (2023) EN 14322
IBU (2023): PCR Part B: Requirements on the EPD for wood­ EN 14322:2021, Wood­based panels – Melamine faced boards
based panels. Version 2019/01, for interior uses – Definitions, requirements and classification.
Institut Bauen und Umwelt, Berlin.
EN 14964
Standards and legal documents EN 14964:2006, Rigid underlays for discontinuous roofing –
Definitions and characteristics.
ASTM D6007
ASTM D6007­14, Standard Test Method for Determining EN 15804
Formaldehyde Concentrations in Air from Wood Products Using EN 15804+A2:2019 + AC:2021, Sustainability of construction
a Small­Scale Chamber. works ­ Environmental product declarations ­ Core rules for the
product category construction products.
EN 310
EN 310:1993, Wood­based panels – Determination of modulus EN 16485
of elasticity in bending and of bending strength. EN 16485:14­07, Round and sawn timber – Environmental
Product Declarations – Product category rules for wood and
EN 316 wood­based products for use in construction.
EN 316:2009, Wood fibre boards – Definition, classification and
symbol. ISO 9001
ISO 9001:2015, Quality management systems – Requirements.
EN 317
EN 317:1993, Particleboards and Fibreboards – Determination ISO 14001
of swelling in thickness after immersion in water. ISO 14001:2015, Environmental management systems –
Requirements with guidance for use.
EN 319
EN 319:1993, Particleboards and fibreboards – Determination ISO 14025
of tensile strength perpendicular to the plane of the board. ISO 14025:2006­07, Environmental labels and declarations –
Type III Environmental declarations – Principles and
EN 322 procedures.
EN 322:1993, Wood­based panels – Determination of moisture
content. ISO 14044
EN ISO 14044:2006­07, Environmental management – Life
EN 323 cycle assessment – Requirements and guidance (ISO
EN 323:1993, Wood­based panels – Determination of density. 14044:2006); German and English versions EN ISO
14044:2006.
EN 324
EN 324­1:1993, Wood­based panels – Determination of ISO 16000
dimensions of boards – Determination of thickness, width and ISO 16000­11:2006, Indoor air – Part 11: Determination of the
length. emission of volatile organic compounds from building products
EN 324­2:1993, Wood­based panels – Determination of and furnishing – Sampling, storage of samples and preparation
dimensions of boards – Determination of squareness and edge of test specimens.
straightness.
ISO 16895
EN 622 ISO 16895­1:2008, Wood­based panels – Dry­process
EN 622­1:2003, Fibreboards – Specifications – Part 1: General fibreboard – Part 1: Classifications.
requirements. ISO 16895­2:2010, Wood­based panels – Dry­process
EN 622­5:2009, Fibreboards – Specifications – Part 5: fibreboard – Part 2: Requirements.
Requirements for dry process boards (MDF).
ISO 45001
EN 717-1 ISO 45001:2018­06, Occupational health and safety
EN 717­1:2005­01, Wood­based panels – Determination of management systems – Requirements with guidance for use.
formaldehyde release – Formaldehyde emission by the
chamber method.
10 Environmental Product Declaration ­ Sonae Arauco, S.A. ­ Medium density fibreboard (MDF), coated
ISO 50001 European Parliament and of the Council.
ISO 50001:2018, Energy management systems –
Requirements with guidance for use. Regulation on the European Waste List (Waste index)
http://www.gesetze­im­internet.de/avv/anlage.html
ECHA-List
The Candidate List of substances of very high concern ChemVerbotsV, Chemikalien­Verbotsverordnung (German
published by the European Chemicals Agency (ECHA), Regulation on the Prohibition of Chemicals, from 14 October
Helsinki, available via https://echa.europa.eu/nl/­/four­ 1993).
newsubstances­added­to­the­candidate­list
Additional references
Regulation on biocidal products
REGULATION (EU) No 528/2012 OF THE EUROPEAN BBSR 2017
PARLIAMENT AND OF THE COUNCIL of 22 May 2012 Bundesinstitut für Bau­, Stadt­ und Raumforschung Service Life
concerning the making available on the market and use of of Building Components; version 24.02.2017.
biocidal products.
https://www.nachhaltigesbauen.de/fileadmin/pdf/Nutzungsdauer_Bauteile/BNB_Nutzungsdauern_von_Bauteilen_2017­
Regulation (EU) Nr. 305/2011(CPR) 2­24.pdf
REGULATION (EU) No 305/2011 OF THE EUROPEAN
PARLIAMENT AND OF THE COUNCIL of 9 March 2011 laying ecoinvent 3.8
down harmonised conditions for the marketing of construction LCA database ecoinvent v3.8, 12/2021. ecoinvent, Zürich.
products and repealing Council Directive 89/106/EEC.
Weidema et al. (2013)
COUNCIL REGULATION (EU) No 333/2011 Weidema, B., C. Bauer, R. Hischier, C. Mutel, T. Nemecek, J.
COUNCIL REGULATION (EU) No 333/2011 of 31 March 2011 Reinhard, C.O. Vadenbo, G. Wernet (2013): Overview and
establishing criteria determining when certain types of scrap methodology, Data quality guideline for the ecoinvent database
metal cease to be waste under Directive 2008/98/EC of the version 3. ecoinvent report no. 1 (v3), St. Gallen (CH).
11 Environmental Product Declaration ­ Sonae Arauco, S.A. ­ Medium density fibreboard (MDF), coated
Publisher
Institut Bauen und Umwelt e.V. +49 (0)30 3087748­ 0
Hegelplatz 1 info@ibu­epd.com
10117 Berlin www.ibu­epd.com
Germany
Programme holder
Institut Bauen und Umwelt e.V. +49 (0)30 3087748­ 0
Hegelplatz 1 info@ibu­epd.com
10117 Berlin www.ibu­epd.com
Germany
Author of the Life Cycle Assessment
Dr. Frank Werner ­ Umwelt & Entwicklung + 41 (0)44 241 39 06
Kammelenbergstrasse 30 frank@frankwerner.ch
9011 St. Gallen http://www.frankwerner.ch/
Switzerland
Owner of the Declaration
Sonae Arauco, S.A. (+34) 918 070 701
Calle Ulises 26­18 products@sonaearauco.com
28043 Madrid www.sonaearauco.com
Spain
12 Environmental Product Declaration ­ Sonae Arauco, S.A. ­ Medium density fibreboard (MDF), coated
