ENVIRONMENTAL PRODUCT DECLARATION
as per ISO 14025 and EN 15804+A2
Owner of the Declaration DBC, EFCC, FEICA, IVK
Programme holder Institut Bauen und Umwelt e.V. (IBU)
Publisher Institut Bauen und Umwelt e.V. (IBU)
Declaration number EPD-DBC-20220147-IBF1-EN
Issue date 08.06.2022
Valid to 07.06.2027
Dispersion-based products, group 2
DBC - Deutsche Bauchemie e.V.
EFCC - European Federation for Construction Chemicals
FEICA - Association of the European Adhesive and Sealant Industry
IVK - Industrieverband Klebstoffe e.V.
www.ibu-epd.com | https://epd-online.com
Umwelt Produktdeklaration Name des Herstellers – Name des Produkts
1. General Information
DBC - Deutsche Bauchemie e.V. Dispersion-based products, group 2
EFCC - European Federation for
Construction Chemicals
FEICA - Association of the European
Adhesive and Sealant Industry
IVK - Industrieverband Klebstoffe e.V.
Programme holder Owner of the declaration
IBU – Institut Bauen und Umwelt e.V. DBC, Mainzer Landstr. 55, D-60329 Frankfurt a.M.
Hegelplatz 1 EFCC, 172 Boulevard du Triomphe, B-1160 Brussels
10117 Berlin FEICA, Rue Belliard 40, B-1040 Brussels
Germany IVK, Völklingerstr. 4, D-40219 Düsseldorf
Declaration number Declared product / declared unit
EPD-DBC-20220147-IBF1-EN 1 kg / 1 kg; density 1,000 - 1,500 kg/m³
This declaration is based on the product Scope:
category rules: This verified EPD entitles the holder to bear the symbol
Dispersion adhesives and primers for floor coverings, of the Institut Bauen und Umwelt e.V. It exclusively
01.2019 applies for products produced in Europe and for a
(PCR checked and approved by the SVR) period of five years from the date of issue. This EPD
may be used by members of DBC, EFCC, FEICA and
IVK and their members provided it has been proven
Issue date
that the respective product can be represented by this
08.06.2022
EPD. For this purpose, a guideline is available at the
secretariats of the four associations. The members of
Valid to the associations are listed on the respective websites.
07.06.2027
The owner of the declaration shall be liable for the
underlying information and evidence; the IBU shall not
be liable with respect to manufacturer information, life
cycle assessment data and evidences.
The EPD was created according to the specifications
of EN 15804+A2. In the following, the standard will be
simplified as EN 15804.
Verification
The standard EN 15804 serves as the core PCR
Independent verification of the declaration and data
according to ISO 14025:2011
Dipl. Ing. Hans Peters internally x externally
(chairman of Institut Bauen und Umwelt e.V.)
Dr. Alexander Röder Matthias Schulz
(Managing Director Institut Bauen und Umwelt e.V.)) (Independent verifier)
2. Product
2.1 Product description/Product definition their life expectancy. The product displaying the
This EPD comprises dispersion-based products with a highest environmental impacts within the class of
Volatile Organic Compound (VOC) content ≤1 % (VOC dispersion-based products considered was used as a
definition according to Decopaint Directive). The representative product for calculating the Life Cycle
products typically consist of organic binding agents Assessment results (worst-case approach).
based on synthetic and/or natural resins, mineral fillers
such as chalk as well as water and smaller volumes of For the placing on the market in the European
auxiliaries (thickening agents, defoaming agents, Union/European Free Trade Association (EU/EFTA)
surface-active agents, preservatives etc.). They dry with the exception of Switzerland) products falling
physically through evaporation of the water contained under the Regulation (EU) No 305/2011 (CPR) need a
therein. They comply with manifold, often specific, Declaration of Performance taking into consideration
functions in the construction, furnishing and repair of either the relevant harmonised European standard or
buildings. Using dispersion-based products decisively the European Technical Assessment and the CE
improves the fitness for use of structures and extends
2 Environmental Product Declaration DBC, EFCC, FEICA, IVK – Dispersion-based products, group 2
marking. For the application and use of the products parquet: The test procedures and requirements of the
the respective national provisions apply. EN ISO 17178 have to be fulfilled.
2.2 Application Module 2: Dispersion-based tile adhesive
Dispersion-based products are used for the following The requirements on essential characteristics
applications: according to EN 12004, must be maintained. These
are:
Module 1: Dispersion adhesives, fixatives, Tensile adhesion strength after dry storage (EN 12004-
precoatings and primers for floor coverings and 2)
parquet flooring -Tensile adhesion strength after water immersion (EN
Adhesives for, e.g. tufted carpets with various 12004-2)
backings, woven textile coverings, fibre-bonded and -Tensile adhesion strength after heat ageing (EN
natural fibre coverings, resilient coverings (PVC, 12004)
rubber, PVC-free luxury vinyl tiles), linoleum, insulating -Tensile adhesion strength after freeze/thaw cycles
bases and underlays, parquet, laminate and wood (EN 12004-2)
blocks on surfaces ready for laying. The products are -Open time: Tensile strength (EN 12004-2)
suitable for normal wear in residential and commercial Further essential characteristics in accordance with the
areas, also on heated floor constructions. manufacturer's technical documentation
Module 2: Dispersion-based tile adhesive Module 3: Dispersion-based adhesives and
Products for bonding ceramic tiles and paving as well sealants
as natural stone for internal and external installations Performance characteristics in accordance with the
on walls, floors and ceilings manufacturer's technical documentation / declaration
of performance
Module 3: Dispersion-based adhesives and
sealants Module 4: Dispersion-based products for
As structural adhesives and sealants: structural and waterproofing of buildings
repair adhesives, dispersion filler compounds, joint The minimum requirement of EAD 030352-00-0503 -
sealants Liquid applied watertight covering kits for wet room
floors and/or walls- must be maintained. The essential
Module 4: Dispersion-based products for characteristics are to be specified in accordance with
waterproofing of buildings the European technical assessment (ETA,
Products for waterproofing floors and/or walls in wet specification no.).
rooms inside buildings
Module 5: Dispersion-based primers and bonding
Module 5: Dispersion-based primers and bonding agents for concrete and floor screeds
agents for concrete and floor screeds Performance characteristics in accordance with the
Products to improve the adhesion of e.g. self-levelling manufacturer's technical documentation
compounds or repair mortars on absorbent cement
and calcium sulphate screeds, concrete, dry Module 6: Dispersion-based products for surface
construction boards protection of concrete
The requirements on essential characteristics for all
Module 6: Dispersion-based products for surface intended uses in accordance with EN 1504-2, Tables 1
protection of concrete and 5, must be maintained. These are:
To increase the durability of concrete and reinforced - Permeability to CO (EN 1062-6)
2
steel structures as well as for new concrete and for - Water vapour permeability (EN ISO 7783-1/-2)
maintenance and repair work (for areas without vehicle - Capillary absorption and permeability to water (EN
traffic) 1062-3)
- Adhesion strength by pull-off test (EN 1542)
Module 7: Dispersion-based primers and barrier Further essential characteristics in accordance with the
coatings manufacturer's technical documentation / declaration
Products to protect a substrate from e.g. the immersion of performance
of water, thus preventing degradation, corrosion or
damage Module 7: Dispersion-based primers and barrier
coatings
2.3 Technical Data The requirements of the Decopaint Directive must be
The density of the products is between 1,00 and 1,50 maintained.
g/cm³, other relevant technical data can be found in the Essential characteristics in accordance with the
manufacturer’s technical documentation. manufacturer's technical documentation / declaration
of performance.
Module 1: Dispersion adhesives, fixatives,
precoatings and primers for floor coverings and
parquet flooring
Dispersion adhesives for floor coverings have to
comply with the requirements of the EN ISO 22636.
The mechanical requirements of EN ISO 22636 don’t
apply to fixatives; their strengths are lower in 2.4 Delivery status
accordance with their specifications. The performance Liquid or pasty in containers made of plastic or metal.
characteristics of precoatings and primers are subject Typical container sizes contain 1 to 30 kg, usually 10
to the manufacturer's technical documentation / to 20 kg of product on pallets. For larger applications,
declaration of performance. Dispersion adhesives for vats with approx. volumes of 200 kg (litres) or IBCs
3 Environmental Product Declaration DBC, EFCC, FEICA, IVK – Dispersion-based products, group 2
(intermediate bulk containers) with a capacity of 1 batches or a series of individual batches, and filled into
tonne (m³) or more are also used. A plastic container the delivery containers.
was modelled for the Life Cycle Assessment.
2.7 Environment and health during
2.5 Base materials/Ancillary materials manufacturing
Dispersion-based products usually comprise at least As a general rule, no particular environmental or health
one synthetic resin dispersion, natural or synthetic protection measures other than those specified by law
resins dispersed in water, mineral fillers (e.g. chalk) are necessary.
and/or pigments. Auxiliaries such as thickening agents,
defoaming agents, surface-active and dispersing 2.8 Product processing/Installation
agents as well as preservatives are used to fine-tune Dispersion based products are processed on site using
the product features. Typically, the products covered suitable tools, usually by hand. The products are
by this EPD contain the following range of base applied by trowelling/knife-coating, painting, rolling or
materials and auxiliaries (% by mass): spraying. Precautions for safe handling and storage
- Synthetic polymer dispersion (solids portion): 5 - 65 (e.g. air exchange, exhaust ventilation, personal
- Natural resins, natural resin derivatives: 0 - 25 protective measures, conditions for safe storage) must
- Mineral fillers: 0 - 60 be observed in accordance with the information on the
- Pigments: 0 - 35 safety data sheet.
- Water: 15 - 95 Depending on the application and product
- Auxiliaries: 1 - 5 specifications, between 50 and 1,500 g/m² are applied.
- Thickening agents: < 3
- Dispersing agents / Emulsifying agents: < 2 2.9 Packaging
- Wetting agent: 2 A detailed description of packaging is provided in
- Other: 0 - 2 section 2.4. Empty containers and clean foils can be
- VOC according to Decopaint Directive: <1 % recycled.
(mandatory)
These ranges are average values and the composition
of products complying with the EPD can deviate from 2.10 Condition of use
these concentration levels in individual cases. More During the use phase, dispersion-based products are
detailed information is available in the respective existent as hardened film. They are long-lasting
manufacturer's documentation (e.g. product data products which protect our buildings in the form of
sheets). adhesives, primers, coatings or sealants as well as
make an essential contribution towards their
Note: For companies to declare their products within appearance, function and sustainability.
the scope of this EPD it is not sufficient to simply
comply with the product composition shown above. 2.11 Environment and health during use
The application of this EPD is only possible for Option 1 – Products for applications outside
member companies of DBC, EFCC, FEICA, and IVK indoor areas with permanent stays by people
member associations and only for specific formulations No risks are known for water, air and soil if the
with a total score below the declared maximum score products are used as designated.
for a product group according to the associated Option 2 – Products for applications inside indoor
guidance document. areas with permanent stays by people
When used in indoor areas with permanent stays by
people, evidence of the emission performance of
1. substances from the “Candidate List of construction products in contact with indoor air must be
Substances of Very High Concern for submitted according to national requirements (see
Authorisation” (SVHC) chapter 7). No further influences by emissions on the
If this product contains substances listed in the environment and health are known.
candidate list (latest version) exceeding 0.1
percentage by mass, the relevant information can be 2.12 Reference service life
found in the safety data sheet of the relevant product Dispersion-based products fulfill manifold, often
covered by this model EPD. specific, functions in the construction or refurbishment
2. CMR substances in categories 1A and 1B of building structures. They decisively improve the
If this product contains other carcinogenic, mutagenic, usability of building structures and significantly extend
reprotoxic (CMR) substances in categories 1A or 1B their original service lives. The anticipated reference
which are not on the candidate list, exceeding 0.1 service life depends on the specific installation
percentage by mass, the relevant information can be situation and the exposure associated with the product.
found in the safety data sheet of the relevant product It can be influenced by weathering as well as
covered by this model EPD. mechanical or chemical load.
3. Biocide products added to the construction
product
If this construction product contains biocide products, 2.13 Extraordinary effects
the active substances, information on the
concentration and/or concentration range, the product Fire
type together with information on their hazardous In terms of the volumes applied, dispersion based
properties are listed in the safety data sheet of the products have no or only a marginal influence on the
respective product. fire performance characteristics of the building
structure in which they have been installed.
2.6 Manufacture
Dispersion-based products are usually mixed Water
discontinuously in batch mode, i.e. in individual
4 Environmental Product Declaration DBC, EFCC, FEICA, IVK – Dispersion-based products, group 2
Dispersion-based products are water-resistant only to
a certain degree and their strength can deteriorate
when exposed to water for longer periods (of time); 2.15 Disposal
detaching from the surface is possible in a worst-case The low amounts of a dispersion-based product
scenario. The components of dispersion-based applied to a construction product will not interfere with
products are not hazardous to water or only slightly the disposal/recycling of this.
hazardous to water. Owing to the overall low volumes Hardened product residue mechanically removed from
of dispersion-based products used on buildings, no substrates must be disposed of as
relevant contribution towards environmental damage commercial/construction waste. The following waste
can be anticipated by buildings featuring dispersion- codes according to the European List of Waste
based products in the event of extraordinary exposure (2000/532/EC) can apply:
to water. Hardened product residue:
080112 Paint and varnish waste with the exception of
Mechanical destruction that covered by 08 01 11
The mechanical destruction of dispersion-based 080410 Adhesive and sealant compound waste with
products does not lead to any decomposition products the exception of that covered by 08 04 09
which are harmful to the environment or health.
2.14 Re-use phase 2.16 Further information
According to present knowledge, no environmentally More information is available on the manufacturer's
hazardous effects in terms of landfilling are to be product or safety data sheets and is available on the
generally anticipated through dismantling and recycling manufacturer's websites or on request. Valuable
components to which dispersion-based products have technical information is also available on the
been applied and on which they have dried. associations' websites.
3. LCA: Calculation rules
3.1 Declared Unit The building deconstruction (demolition process) takes
This EPD refers to the declared unit of 1 kg of place in the C1 module which considers energy
dispersion-based product, group 2; applied into the production and consumption in terms of diesel and all
building with a density of 1,000 - 1,500 kg/m^3 in the emissions connected with the fuel-burning process
accordance with the IBU PCR part B for dispersion to run the machines. After the demolition, the product
adhesives and primers for floor coverings. is transported to the end-of-life processing (C2
The results of the Life Cycle Assessment provided in module) where all the impacts related to the transport
this declaration have been selected from the product processes are considered. For precautionary principle
with the highest environmental impact (worst-case and as a worst-case scenario, thermal treatment is the
scenario). only end of life scenario considered. This is modelled
Depending on the application, a corresponding by the incineration process (module C3) where the
conversion factor such as the density to convert product ends its life cycle.
volumetric use to mass must be taken into Module D accounts for potential benefits that are
consideration. beyond the defined system boundaries. Credits are
generated during the incineration of wastes and related
The Declaration type is according to EN 15804: Cradle electricity produced that are occurring in the A5
to gate with options, modules C1–C3, and module D module.
(A1–A3, C, D) and additional modules (A4-A5).
3.3 Estimates and assumptions
Declared unit For this EPD formulation and production data defined
Name Value Unit and collected by FEICA were considered. Production
Declared unit 1 kg waste was assumed to be disposed of by incineration
1,000- without credits as a worst case.
Gross density kg/m^3
1,500 An average of plastic containers and wooden pallets
was considered in the LCA.
3.4 Cut-off criteria
3.2 System boundary All raw materials submitted for the formulations and
Modules A1, A2 and A3 are taken into consideration in production data were taken into consideration.
the LCA: The manufacture of machinery, plant and other
- A1 Production of preliminary products infrastructure required for the production of the
- A2 Transport to the plant products under review was not taken into consideration
- A3 Production incl. provision of energy, production of in the LCA.
packaging as well as auxiliaries and consumables and Transport of packaging materials is excluded.
waste treatment
- A4 Transport to site 3.5 Background data
- A5 Installation, product applied into the building Data from the GaBi database SP40 (2020) was used
during A5 phase operations and packaging disposal. as background data.
The end of life for the packaging material considered is
described below: 3.6 Data quality
-Incineration, for materials like plastic and wood. Representative products were applied for this EPD and
-C1-C2-C3-D the product in the group displaying the highest
environmental impact was selected for calculating the
5 Environmental Product Declaration DBC, EFCC, FEICA, IVK – Dispersion-based products, group 2
LCA results. The background datasets used are less 3.8 Allocation
than 4 years old. Mass allocation has been applied when primary data
Production data and packaging are based on details have been used and implemented into the LCA model.
provided by the manufacturer. The formulation used for
evaluation refers to a specific product. 3.9 Comparability
The data quality of the background data is considered Basically, a comparison or an evaluation of EPD data
to be good. is only possible if all the data sets to be compared
were created according to EN 15804 and the building
3.7 Period under review context, respectively the product-specific
Representative formulations are valid for 2021. characteristics of performance, are taken into account.
The GaBi database SP40 (2020) was used.
4. LCA: Scenarios and additional technical information
Characteristic product properties
Information on biogenic Carbon
The packaging material contains biogenic carbon
content which is presented below.
Information on describing the biogenic Carbon
Content at factory gate
Name Value Unit
Biogenic Carbon Content in product - kg C
Biogenic Carbon Content in
0.016 kg C
accompanying packaging
For the preparation of building life cycle assessments,
it must be taken into account that in module A5
(installation in the building) the biogenic amount of CO
2
(0.016 kg C *3.67 = 0.059 kg CO -eq.) of the
2
packaging bound in module A1-A3 is mathematically
booked out.
Transport to the building site (A4)
Name Value Unit
Transport distance 1000 km
Gross weight 34 - 40 t
Payload capacity 27 t
Installation into the building (A5)
Name Value Unit
Other resources for packaging material 0.067 kg
Material loss 0.01 kg
Material loss regards the amount of product not used
during the application phase into the building. This
amount is 1% of the product, impacts related to the
production of this part are charged to the A5 module.
This percentage is considered as waste to disposal
and impacts of its end of life have been considered in
the LCA model and declared in A5.
End of life (C1-C3)
Name Value Unit
Collected as mixed construction waste 1 kg
Incineration 1 kg
6 Environmental Product Declaration DBC, EFCC, FEICA, IVK – Dispersion-based products, group 2
5. LCA: Results
DESCRIPTION OF THE SYSTEM BOUNDARY (X = INCLUDED IN LCA; ND = MODULE OR INDICATOR NOT
DECLARED; MNR = MODULE NOT RELEVANT)
BENEFITS AND
CONSTRUCTI LOADS
PRODUCT STAGE ON PROCESS USE STAGE END OF LIFE STAGE BEYOND THE
STAGE SYSTEM
BOUNDARIES
7 Environmental Product Declaration DBC, EFCC, FEICA, IVK – Dispersion-based products, group 2
lairetam
waR
ylppus tropsnarT
gnirutcafunaM
eht
morf
tropsnarT
etis
eht
ot
etag
ylbmessA esU
ecnanetniaM
riapeR
tnemecalpeR tnemhsibrufeR
ygrene
lanoitarepO esu
retaw
lanoitarepO esu
noitcurtsnoc-eD
noitilomed tropsnarT
gnissecorp
etsaW
lasopsiD -esueR -yrevoceR -gnilcyceR laitnetop
A1 A2 A3 A4 A5 B1 B2 B3 B4 B5 B6 B7 C1 C2 C3 C4 D
X X X X X ND ND MNR MNR MNR ND ND X X X ND X
RESULTS OF THE LCA - ENVIRONMENTAL IMPACT according to EN 15804+A2: 1 kg of dispersion-based
product, group 2
Core Indicator Unit A1-A3 A4 A5 C1 C2 C3 D
GWP-total [kg CO2-Eq.] 2.00E+0 5.11E-2 1.80E-1 2.79E-4 1.24E-2 9.45E-1 -3.98E-1
GWP-fossil [kg CO2-Eq.] 2.05E+0 5.06E-2 9.49E-2 2.66E-4 1.18E-2 4.29E-1 -3.97E-1
GWP-biogenic [kg CO2-Eq.] -3.96E-2 1.48E-4 8.54E-2 1.24E-5 5.42E-4 5.15E-1 -8.96E-4
GWP-luluc [kg CO2-Eq.] 8.17E-4 4.10E-4 9.68E-6 6.39E-9 2.79E-7 3.50E-5 -2.51E-4
ODP [kg CFC11-Eq.] 3.53E-14 6.08E-18 3.70E-16 2.84E-20 1.24E-18 3.02E-16 -3.72E-15
AP [mol H+-Eq.] 8.99E-3 1.52E-4 1.14E-4 3.60E-6 3.73E-5 5.25E-4 -5.26E-4
EP-freshwater [kg P-Eq.] 2.85E-5 1.54E-7 2.88E-7 5.75E-11 2.51E-9 1.04E-7 -4.62E-7
EP-marine [kg N-Eq.] 1.70E-3 6.75E-5 2.42E-5 1.63E-6 1.72E-5 2.01E-4 -1.39E-4
EP-terrestrial [mol N-Eq.] 1.95E-2 7.56E-4 3.08E-4 1.79E-5 1.89E-4 2.52E-3 -1.49E-3
POCP [kg NMVOC-Eq.] 6.25E-3 1.33E-4 8.24E-5 4.91E-6 3.39E-5 5.22E-4 -4.02E-4
ADPE [kg Sb-Eq.] 7.32E-7 3.63E-9 7.60E-9 8.06E-12 3.52E-10 4.62E-9 -6.06E-8
ADPF [MJ] 4.44E+1 6.73E-1 4.75E-1 3.81E-3 1.66E-1 5.52E-1 -6.70E+0
[m³ world-Eq
WDP 6.36E-2 4.52E-4 1.70E-2 5.27E-7 2.30E-5 1.57E-1 -3.70E-2
deprived]
GWP = Global warming potential; ODP = Depletion potential of the stratospheric ozone layer; AP = Acidification potential of land and water; EP =
Caption Eutrophication potential; POCP = Formation potential of tropospheric ozone photochemical oxidants; ADPE = Abiotic depletion potential for non-
fossil resources; ADPF = Abiotic depletion potential for fossil resources; WDP = Water (user) deprivation potential
RESULTS OF THE LCA - INDICATORS TO DESCRIBE RESOURCE USE according to EN 15804+A2: 1 kg of
dispersion-based product, group 2
Indicator Unit A1-A3 A4 A5 C1 C2 C3 D
PERE [MJ] 6.19E+0 3.79E-2 6.58E-1 1.20E-5 5.25E-4 9.36E-2 -1.32E+0
PERM [MJ] 5.85E-1 0.00E+0 -5.85E-1 0.00E+0 0.00E+0 0.00E+0 0.00E+0
PERT [MJ] 6.77E+0 3.79E-2 7.35E-2 1.20E-5 5.25E-4 9.36E-2 -1.32E+0
PENRE [MJ] 2.93E+1 6.74E-1 1.43E+0 3.81E-3 1.67E-1 1.48E+1 -6.70E+0
PENRM [MJ] 1.52E+1 0.00E+0 -9.53E-1 0.00E+0 0.00E+0 -1.42E+1 0.00E+0
PENRT [MJ] 4.44E+1 6.74E-1 4.76E-1 3.81E-3 1.67E-1 5.52E-1 -6.70E+0
SM [kg] 0.00E+0 0.00E+0 0.00E+0 0.00E+0 0.00E+0 0.00E+0 0.00E+0
RSF [MJ] 0.00E+0 0.00E+0 0.00E+0 0.00E+0 0.00E+0 0.00E+0 0.00E+0
NRSF [MJ] 0.00E+0 0.00E+0 0.00E+0 0.00E+0 0.00E+0 0.00E+0 0.00E+0
FW [m³] 1.54E-2 4.38E-5 5.38E-4 2.16E-8 9.41E-7 3.70E-3 -1.53E-3
PERE = Use of renewable primary energy excluding renewable primary energy resources used as raw materials; PERM = Use of
renewable primary energy resources used as raw materials; PERT = Total use of renewable primary energy resources; PENRE = Use of
non-renewable primary energy excluding non-renewable primary energy resources used as raw materials; PENRM = Use of non-
Caption
renewable primary energy resources used as raw materials; PENRT = Total use of non-renewable primary energy resources; SM = Use
of secondary material; RSF = Use of renewable secondary fuels; NRSF = Use of non-renewable secondary fuels; FW = Use of net fresh
water
RESULTS OF THE LCA – WASTE CATEGORIES AND OUTPUT FLOWS according to EN 15804+A2:
1 kg of dispersion-based product, group 2
Indicator Unit A1-A3 A4 A5 C1 C2 C3 D
HWD [kg] 1.51E-8 3.14E-8 1.87E-10 3.70E-13 1.62E-11 1.77E-9 -2.66E-9
NHWD [kg] 2.75E-1 1.03E-4 4.97E-3 3.90E-7 1.70E-5 1.36E-1 -2.94E-3
RWD [kg] 1.09E-3 8.34E-7 1.27E-5 4.09E-9 1.79E-7 2.51E-5 -4.51E-4
CRU [kg] 0.00E+0 0.00E+0 0.00E+0 0.00E+0 0.00E+0 0.00E+0 0.00E+0
MFR [kg] 0.00E+0 0.00E+0 0.00E+0 0.00E+0 0.00E+0 0.00E+0 0.00E+0
MER [kg] 0.00E+0 0.00E+0 0.00E+0 0.00E+0 0.00E+0 0.00E+0 0.00E+0
EEE [MJ] 0.00E+0 0.00E+0 2.77E-1 0.00E+0 0.00E+0 0.00E+0 0.00E+0
EET [MJ] 0.00E+0 0.00E+0 5.01E-1 0.00E+0 0.00E+0 0.00E+0 0.00E+0
HWD = Hazardous waste disposed; NHWD = Non-hazardous waste disposed; RWD = Radioactive waste disposed; CRU = Components
Caption for re-use; MFR = Materials for recycling; MER = Materials for energy recovery; EEE = Exported electrical energy; EET = Exported
thermal energy
RESULTS OF THE LCA – additional impact categories according to EN 15804+A2-optional:
1 kg of dispersion-based product, group 2
Indicator Unit A1-A3 A4 A5 C1 C2 C3 D
[Disease
PM ND ND ND ND ND ND ND
Incidence]
[kBq U235-
IRP ND ND ND ND ND ND ND
Eq.]
ETP-fw [CTUe] ND ND ND ND ND ND ND
HTP-c [CTUh] ND ND ND ND ND ND ND
HTP-nc [CTUh] ND ND ND ND ND ND ND
SQP [-] ND ND ND ND ND ND ND
PM = Potential incidence of disease due to PM emissions; IR = Potential Human exposure efficiency relative to U235; ETP-fw = Potential
Caption comparative Toxic Unit for ecosystems; HTP-c = Potential comparative Toxic Unit for humans (cancerogenic); HTP-nc = Potential
comparative Toxic Unit for humans (not cancerogenic); SQP = Potential soil quality index
Potential Human exposure efficiency relative to U235, Disclaimer 1 – This impact category deals mainly with the
eventual impact of low dose ionizing radiation on human health of the nuclear fuel cycle. It does not consider
effects due to possible nuclear accidents, occupational exposure or radioactive waste disposal in underground
facilities. Potential ionizing radiation from the soil, radon and (from) some construction materials, is also not
measured by this indicator.
ADP minerals & metals, ADP fossil, WDP, ETF-fw, HTP-c, HTP-nc, SQP, Disclaimer 2 – The results of this
environmental impact indicator shall be used with care as the uncertainties on these results are high or as there is
limited experience with the indicator.
Additional environmental impact indicators (suggested by EN15804, table 4) are not declared in the EPD. The
results of this environmental impact indicator shall be used with care as the uncertainties on these results are high
and as there is limited experience with the indicator (see ILCD classification in EN 15804, table 5). For this
reason, results based on these indicators are not considered suitable for a decision-making process and are thus
not declared in the EPD.
6. LCA: Interpretation
The majority of impacts are associated with the renewable energy resources required for the
production phase (A1-A3). The most significant generation and supply of electricity. It should be noted
contribution to the production phase impacts is the that Primary Energy Demand – Renewable (PERT)
upstream production of raw materials as the main generally represents a small percentage of the
driver. Another contributor in the production phase, in production phase primary energy demand with the bulk
the category of Photochemical ozone formation of the demand coming from non-renewable energy
(POCP), is the plastic used as a packaging material. resources.
Emissions associated with the manufacturing of Transportation to the construction site (A4) and the
products also have some influence on Ozone installation process (A5) make a low contribution to all
Depletion Potential (ODP) in the production phase. In impacts. Climate change from land-use change is the
all EPDs, CO is the most important contributor to only indicator influenced by transport processes, due
2
Global Warming Potential (GWP). For the Acidification to the diesel production used as fuel because part of
Potential (AP), NOx and SO contribute the largest this diesel has been produced from bio-based raw
2
share. materials.
The majority of life cycle energy consumption takes The installation phase influence mainly climate change
place during the production phase (A1-A3). Significant indicators, due to the impact related to the incineration
contributions to Primary Energy Demand – Non- processes used for packaging waste treatment and
renewable (PENRT) come from the energy resources residual product treatment (1 % of the total mass).
used in the production of raw materials. The largest The end-of-life phases influence climate change
contributor to Primary Energy Demand – Renewable indicators, due to the thermal treatment process of the
(PERT) impacts comes from the consumption of dispersion-based product occurring in the C3 module.
7. Requisite evidence
any of the existing regulations or in any of the existing
VOC voluntary labelling programs for low-emitting products,
Special tests and evidence have not been carried out as far as these
or provided within the framework of drawing up this (1) include limits for the parameters TVOC, TSVOC,
Model EPD. Some member states require special carcinogens, formaldehyde, acetaldehyde, LCI limits
documentation on VOC emissions into indoor air for for individual substances (including but not limited to
specific areas of application. This documentation, as the European list of harmonized LCIs), and the R-
well as documentation for voluntary VOC labelling, has value;
to be provided separately and is specific to the product (2) base their test methods on EN 16516;
in question. (3) perform testing and apply the limits after 28 days
of storage in a ventilated test chamber, under the
Evidence pertaining to VOC emissions shall show conditions specified in EN 16516; some regulations
- either an attestation of compliance with, and programs also have limits after 3 days, on top of
- or documentation of test data that are required in the 28 days limits;
8 Environmental Product Declaration DBC, EFCC, FEICA, IVK – Dispersion-based products, group 2
(4) express the test results as air concentrations in - Each carcinogen: 1 µg/m³
the European Reference Room, as specified in EN - Formaldehyde: 100 µg/m³
16516. - LCI: different per substance involved
- R-value: 1 (meaning that, in total, 100 % of the
Examples of such regulations are the Belgian Royal combined LCI values must not be exceeded).
Decree C-2014/24239, or the German AgBB/ ABG. Informative Annexes (2 tables):
Examples of such voluntary labelling programs are Table 1 shown below is an overview of the most
EMICODE, Blue Angel or Indoor Air Comfort. relevant regulations and specifications as of October
2021, as regards requirements after 3 days of storage
Relevant test results shall be produced either by an in a ventilated test chamber.
ISO 17025 accredited commercial test lab or by a Table 2 provides an overview of the most relevant
qualified internal test lab of the manufacturer. regulations and specifications as of October 2021, as
Examples for the applied limits after 28 days of storage regards requirements after 28 days of storage in a
in a ventilated test chamber are: ventilated test chamber. Some details may be missing
- TVOC: 1000 µg/m³ in the table due to lack of space. Values given
- TSVOC: 100 µg/m³ represent maximum values/limits.
8. References
EN 1062-3
EN 1062-3:2008-04, Paints and varnishes - Coating EN 1062-6
materials and coating systems for exterior masonry EN 1062-6:2002-10, Paints and varnishes - Coating
and concrete - Part 3: Determination of liquid water materials and coating systems for exterior masonry
permeability
9 Environmental Product Declaration DBC, EFCC, FEICA, IVK – Dispersion-based products, group 2
and concrete - Part 6: Determination of carbon dioxide
permeability 2000/532/EC
Commission decision dated 3 May 2000 replacing
EN 1504-2 decision 94/3/EC on a waste directory in accordance
EN 1504-2:2004-10, Products and systems for the with Article 1 a) of Council Directive 75/442/EEC on
protection and repair of concrete structures - waste and Council decision 94/904/EC on a directory
Definitions, requirements, quality control and of hazardous waste in terms of Article 1, paragraph 4
evaluation of conformity - Part 2: Surface protection of Directive 91/689/EEC on hazardous waste
systems for concrete
Belgian Royal Decree C-2014/24239
EN 1542 Belgisch Staatsblad 8 MEI 2014, p. 60603. —
EN 1542:1999-07, Products and systems for the Koninklijk besluit tot vaststelling van de
protection and repair of concrete structures - Test drempelniveaus voor de emissies naar het
methods - Measurement of bond strength by pull-off binnenmilieu van bouwproducten voor bepaalde
geoogde gebruiken
EN ISO 7783-1/-2
EN ISO 7783-1/-2:2019-02, Paints and varnishes - Blue Angel
Determination of water-vapour transmission properties Environmental label organised by the federal
- Cup method government of Germany www.blauer-engel.de
EN 12004 Candidate list
EN12004:2012, Adhesives for ceramic tiles Candidate List of substances of very high concern for
Authorisation, published in accordance with Article
EN 12004-2 59(10) of the REACH Regulation, ECHA,
EN 12004-2:2017, Adhesives for ceramic tiles - Part 2: www.echa.europa.eu/candidate-list-table
Test methods
CPR
ISO 14025 CPR Regulation (EU) No 305/2011 of the European
DIN EN ISO 14025:2011-10, Environmental labels and Parliament and of the Council of 9 March 2011 laying
declarations — Type III environmental declarations — down harmonised conditions for the marketing of
Principles and procedures construction products and repealing Council Directive
89/106/EEC
EN 15804
EN 15804:2019+A2+AC, Sustainability of construction Decopaint Directive
works — Environmental Product Declarations — Core Directive 2004/42/CE of the European Parliament and
rules for the product category of construction products. the council of 21 April 2004 on the limitation of
emissions of volatile organic compounds due to the
EN 16516 use of organic solvents in certain paints and varnishes
EN 16516:2017 and vehicle refinishing products and amending
Construction products - Assessment of release of Directive 1999/13/EC
dangerous substances - Determination of emissions
into indoor air EMICODE
EMICODE, GEV – Gemeinschaft
EN ISO 17025 Emissionskontrollierte Verlegewerkstoffe, Klebstoffe
EN ISO 17025: 2018-03 und Bauprodukte e. V. (pub.).www.emicode.de
General requirements for the competence of testing
and calibration laboratories GaBi 10 software & documentation
Data base for Life Cycle Engineering LBP, University
EN ISO 17178 of Stuttgart and Sphera, documentation of GaBi 10
EN ISO 17178:2020, Adhesives - Adhesives for data sets http://documentation.gabi-software.com/,
bonding parquet to subfloor - Test methods and 2020
minimum requirements
German AgBB
EN ISO 22636 Committee for Health-related Evaluation of Building
EN ISO 22636:2020, Adhesives - Adhesives for floor Products: health-related evaluation of emissions of
coverings - Requirements for mechanical and electrical volatile organic compounds (VOC and SVOC) from
performance building products; status: June 2012
www.umweltbundesamt.de/produkte/bauprodukte/agb
EAD 030352-00-0503 b.htm
EAD 030352-00-0503:2019-01, Watertight covering
kits for wet room floors and or walls Part 1: Liquid IBU 2021
Applied Coverings with or without wearing surface Part Institut Bauen und Umwelt e.V.: General Instructions
2: Kits based on flexible sheets Part 3: Kits based on for the EPD programme of Institut Bauen und Umwelt
inherently watertight boards e.V. EPD programme. Version 2.0. Berlin: Institut
Bauen und Umwelt e.V., 2021
(EU) No 528/2012 www.ibu-epd.com
Biocidal Products Regulation (EU) No 528/2012 of the
European Parliament and of the Council of 22 May Indoor Air Comfort
2012 concerning the making available on the market Product certification by Eurofins, Hamburg, Germany
and use of biocidal products (current consolidated www.eurofins.com .
version: 2021-06)
10 Environmental Product Declaration DBC, EFCC, FEICA, IVK – Dispersion-based products, group 2
PCR Part A 2006 on the registration, evaluation, approval and
Product Category Rules for Building-Related Products restriction of chemical substances (REACH), for
and Services, Part A: Calculation Rules for the Life establishing a European Agency for chemical
Cycle Assessment and Requirements on the Project substances, for amending Directive 1999/45/EC and
report, Version 1.1, Institut Bauen und Umwelt e.V., for annulment of Directive (EEC) No. 793/93 of the
2021-01 Council, Directive (EC) No. 1488/94 of the
Commission, Guideline 76/769/EEC of the Council and
PCR Part B Guidelines 91/155/EEC, 93/67/EEC, 93/105/EC and
Product Category Rules for Construction Products. 2000/21/EC of the Commission.
Part B: Dispersion adhesives and primers for floor
coverings, Version 1.7, 2019.
REACH
Directive (EG) No. 1907/2006 of the European
Parliament and of the Council dated 18 December
11 Environmental Product Declaration DBC, EFCC, FEICA, IVK – Dispersion-based products, group 2
Publisher
Institut Bauen und Umwelt e.V. Tel +49 (0)30 3087748- 0
Hegelplatz 1 Fax +49 (0)30 3087748- 29
10117 Berlin Mail info@ibu-epd.com
Germany Web www.ibu-epd.com
Programme holder
Institut Bauen und Umwelt e.V. Tel +49 (0)30 - 3087748- 0
Hegelplatz 1 Fax +49 (0)30 – 3087748 - 29
10117 Berlin Mail info@ibu-epd.com
Germany Web www.ibu-epd.com
Author of the Life Cycle
Assessment Tel +49 711 341817-0
Sphera Solutions GmbH Fax +49 711 341817-25
Hauptstraße 111- 113 Mail info@sphera.com
70771 Leinfelden-Echterdingen Web www.sphera.com
Germany
Owner of the Declaration
EFCC - European Federation for Tel +32289720-39
Construction Chemicals Fax +32289720-37
Boulevard du Triomphe 172 Mail info@efcc.be
1160 Brussels Web www.efcc.eu
Belgium
Tel +49 (0)69 2556-1318
Deutsche Bauchemie e.V. Fax +49 (0)69 2556-1319
Mainzer Landstr. 55 Mail info@deutsche-bauchemie.de
60329 Frankfurt Web www.deutsche-bauchemie.de
Germany
Tel +32 (0)267 673 20
FEICA - Association of the Fax +32 (0)267 673 99
European Adhesive and Sealant Mail info@feica.eu
Industry Web www.feica.eu
Rue Belliard 40 box 10
1040 Brussels
Belgium
Tel +49 (0)211 67931-10
Fax +49 (0)211 67931-33
Mail info@klebstoffe.com
Industrieverband Klebstoffe e.V Web www.klebstoffe.com
Völklinger Straße 4
40219 Düsseldorf
Germany
