ENVIRONMENTAL-PRODUCT DECLARATION
as per ISO 14025 and EN 15804+A1
Owner of the Declaration dormakaba International Holding GmbH
Publisher Institut Bauen und Umwelt e.V. (IBU)
Programme holder Institut Bauen und Umwelt e.V. (IBU)
Declaration number EPD-DOR-20200113-CBA2-EN
Issue date 24/08/2020
Valid to 23/08/2025
BEST HD8000
dormakaba
www.ibu-epd.com | https://epd-online.com
General Information
dormakaba BEST HD8000
Programme holder Owner of the declaration
IBU – Institut Bauen und Umwelt e.V. dormakaba International Holding GmbH
Hegelplatz 1 DORMA Platz 1
10117 Berlin 58256 Ennepetal
Germany Germany
Declaration number Declared product / declared unit
EPD-DOR-20200113-CBA2-EN 1 door closer (1 piece) of the BEST HD8000 series
This declaration is based on the product category rules: Scope:
Building Hardware products, 01/08/2021 This EPD refers to a specific door closer manufactured by dormakaba
(PCR checked and approved by the SVR) Production GmbH & Co. KG. The production site is located in Singapore.
The LCA results are valid for the variants HD8016 and HD8056.
Issue date The owner of the declaration shall be liable for the underlying information
and evidence; the IBU shall not be liable with respect to manufacturer
24/08/2020
information, life cycle assessment data and evidences.
The owner of the declaration shall be liable for the underlying information
and evidence; the IBU shall not be liable with respect to manufacturer
Valid to
information, life cycle assessment data and evidences.
23/08/2025
The EPD was created according to the specifications of EN 15804+A1. In
the following, the standard will be simplified as EN 15804 bezeichnet.
Verification
The standard EN 15804 serves as the core PCR
Independent verification of the declaration and data according to ISO
14025:2011
internally X externally
Dipl.-Ing Hans Peters
(chairman of Institut Bauen und Umwelt e.V.)
Florian Pronold Dr.-Ing. Wolfram Trinius,
(Managing Director Institut Bauen und Umwelt e.V.) (Independent verifier)
1 Environmental-Product Declaration - dormakaba - BEST HD8000
Product
Product description/Product definition
The HD8000 series are non-handed surface applied door Example:
closers with adjustable spring power (size 1-6 and size 5-6) and
backcheck that controls opening motion during abusive or
abrupt opening. Supported by a full complement of optional
arms, plates, and brackets, the door closers provide the Technical
flexibility needed to meet the demands of commercial and Data for Locking Cylinders acc. to the classification in EN
institutional applications, including Americans with Disabilities 1303: Performance data of the product with respect to its
Act (ADA) barrierfree accessibility requirements (only size 1-6). characteristics in accordance with the relevant technical
The door closers are available with plastic and metal cover. For provision which can be applied are mentioned above.
the use and application of the product the respective national
provisions at the place of use apply. The standards which can The plant in
be applied are the following: Singapore is certified to the quality management system ISO
9001, which
ensures consistent quality of dormakaba's products.
• ANSI/BHMA 156.4
• ANSI/ICC A117.1 The Environmental Management System in the Singapore
• UL listed product production is certified to ISO 14001 and the Energy
• UL 10C Management to ISO
• ADA compliant (version 1-6) 50001.
Application Base materials/Ancillary materials
The HD8000 series closers are designed for commercial and Name Value Unit
institutional applications, including ADA barrier-free accessibility Steel 62 %
requirements. They are suitable for use on hollow metal, Aluminum 25 %
aluminum
Plastic 4 %
and wood doors and can be used for fire doors.
Oil 4 %
Technical Data Others (Lacquer) 4 %
The door closers have following technical properties:
The products include partial articles which contain substances
listed in
the Candidate List of REACH Regulation 1907/2006/EC (date:
16.01.2020) exceeding 0.1 percentage by mass in the alloy:
• Lead (Pb): 7439-290-1-1 (CAS-No.)
The Candidate List can be found on the ECHA website
address: https://echa.europa.eu/de/home.
Environment and health during use
Reference service life
The reference service life of the HD8000 Series door closers
depends on the traffic pattern and degree of
usage of the door. These closers are rated to ANSI Grade 1,
meaning they
are designed to withstand a minimum of 1,500,000 cycles. The
Please list the Technical Data according to the reference
List in the chapter “Product group specific calculation rules” service life amounts for 20 years.
LCA: Calculation rules
The difference in product weight for the two-door
Declared Unit closer types is approx. 4%. The product with the highest weight
The declared unit of this analysis is one door closer. is
Declared unit declared in this EPD representing the entire product series.
Name Value Unit
For IBU core EPDs (where clause 3.6 is part of the EPD): for
Declared unit 1 piece/product
average EPDs, an estimate of the robustness of the LCA
Conversion factor to 1 kg 0.2427 - values must be made, e.g. concerning variability of the
Mass of declared Product 4.12 kg production process, geographical representativeness and the
2 Environmental-Product Declaration - dormakaba - BEST HD8000
influence of background data and preliminary products D comprises the recycling of metals and gives the recycling
compared to the environmental impacts caused by actual potentials as well as potential benefits from energy substitution.
production.
A5 is declared to ensure the export of biogenic CO2 that is
incorporated in the used packaging materials (paper). Potential
System boundary
benefits from the incineration of packaging materials are also
Type of EPD: declared in module D. The incineration processes in the End-of-
cradle to gate - with options. Life are based on European datasets. The recycling processes
in the End-of-Life are based on European and Global datasets.
The Environmental Product Declaration refers to the production
stage (A1-A3), transport from the gate to construction site (A4), Geographic Representativeness
the end of life stage (C3) and indicates the recycling potential Land or region, in which the declared product system is
which is declared in the module "benefits and loads beyond the manufactured, used or handled at the end of the product´s
product system boundary" (D). lifespan: Singapore
In line with the PCR, A5 is declared to ensure the export of
biogenic CO2 from renewable packaging materials. Comparability
Basically, a comparison or an evaluation of EPD data is only
Modules A1 to A3 include the provision and processing of raw possible if all the data sets to be compared were created
materials as well as the processing of input materials, the according to EN 15804 and the building context, respectively
transport to manufacturer and production site. Module C3 the product-specific characteristics of performance, are taken
includes the incineration of plastics for energy recovery. Module into account.
LCA: Scenarios and additional technical information
addition, it shall be stated that the RSL applies for the reference
Additional technical information for the conditions only.
declared modules.
The same holds for a service life declared by the manufacturer.
Transport to the building site (A4)
Corresponding information related to in-use conditions needs
Name Value Unit
not be provided if a service life taken from the list on service life
Litres of fuel truck (per piece) 0.008 l/100km by BNB is declared.
Transport distance truck 2000 km
Capacity utilisation (including empty runs) 85 % End of life (C1-C4)
Transport distance ship 13000 km Name Value Unit
Recycling 4.12 kg
Installation into the building (A5)
Name ValueUnit Reuse, recovery and/or recycling potentials (D), relevant
Output substances following waste treatment on scenario information
0.25 kg
site (packaging) Name Value Unit
Recycling 100 %
In case a reference service life according to applicable ISO
Collection rate is 100%.
standards is declared then the assumptions and in-use
conditions underlying the determined RSL shall be declared. In
3 Environmental-Product Declaration - dormakaba - BEST HD8000
LCA: Results
The table below
summarizes which modules are declared (as indicated by an "X"), and
which are not declared (as indicated with "MND").
DESCRIPTION OF THE SYSTEM BOUNDARY (X = INCLUDED IN LCA; MND = MODULE NOT DECLARED; MNR = MODULE NOT
RELEVANT)
BENEFITS
AND LOADS
CONSTRUCTION
BEYOND
PRODUCT STAGE PROCESS USE STAGE END OF LIFE STAGE
THE SYSTEM
STAGE
BOUNDARIE
S
la ire ta m w a Ry lp p u s tro p s n a rT g n iru tc a fu n a M e h t m o rf tro p s n a rTe tis e h t o t e ta g y lb m e s s A e s U e c n a n e tn ia M ria p e R tn e m e c a lp e R tn e m h s ib ru fe R y g re n e la n o ita re p Oe s u re ta w la n o ita re p Oe s u n o itc u rts n o c -e Dn o itilo m e d tro p s n a rT g n is s e c o rp e ts a W la s o p s iD -e s u e R-y re v o c e R-g n ilc y c e Rla itn e to p
A1 A2 A3 A4 A5 B1 B2 B3 B4 B5 B6 B7 C1 C2 C3 C4 D
X X X X X MND MND MNR MNR MNR MND MND MND MND X MND X
RESULTS OF THE LCA - ENVIRONMENTAL IMPACT according to EN 15804+A1: 1 door closer (4.12kg)
Parameter Unit A1-A3 A4 A5 C3 D
Global warming potential (GWP) kg CO 2 eq 10.4 1.21 0.349 0.689 -3.47
Depletion potential of the stratospheric ozone layer (ODP) kg CFC11 eq 7.71E-10 9.8E-17 8.4E-17 3.74E-16 -7.72E-16
Acidification potential of land and water (AP) kg SO 2 eq 4.22E-02 2.6E-02 7.31E-05 4.57E-04 -8.42E-03
Eutrophication potential (EP) kg PO 43 eq 3.92E-03 2.99E-03 1.38E-05 7E-05 -7.25E-04
Formation potential of tropospheric ozone photochemical oxidants (POCP) kg Ethen eq 3.92E-03 6.56E-04 4.83E-06 1.85E-05 -8.91E-04
Abiotic depletion potential for non fossil resources (ADPE) kg Sb eq 3.29E-04 4.01E-08 6.86E-09 5.58E-08 5.84E-06
Abiotic depletion potential for fossil resources (ADPF) MJ 149 15.9 0.0968 0.307 -31.5
RESULTS OF THE LCA - INDICATORS TO DESCRIBE RESOURCE USE according to EN 15804+A1: 1 door closer (4.12kg)
Parameter Unit A1-A3 A4 A5 C3 D
Renewable primary energy as energy carrier (PERE) MJ 29.702 0.0601 3.717 0.0683 -0.226
Renewable primary energy resources as material utilization (PERM) MJ 3.698 0 -3.698 0 0
Total use of renewable primary energy resources (PERT) MJ 33.4 0.0601 0.0194 0.0683 -0.226
Non renewable primary energy as energy carrier (PENRE) MJ 141.101 15.9 0 19.242 -34
Non renewable primary energy as material utilization (PENRM) MJ 18.899 0 0 -18.899 0
Total use of non renewable primary energy resources (PENRT) MJ 160 15.9 0.113 0.343 -34
Use of secondary material (SM) kg 2.61 0 0 0 0
Use of renewable secondary fuels (RSF) MJ 0 0 0 0 0
Use of non renewable secondary fuels (NRSF) MJ 0 0 0 0 0
Use of net fresh water (FW) m3 0.0488 0.000275 0.00102 0.00245 -0.00927
RESULTS OF THE LCA – WASTE CATEGORIES AND OUTPUT FLOWS according to EN 15804+A1:
1 door closer (4.12kg)
Parameter Unit A1-A3 A4 A5 C3 D
Hazardous waste disposed (HWD) kg 7.23E-06 2.06E-09 2.19E-10 2.06E-09 -2.32E-09
Non hazardous waste disposed (NHWD) kg 0.955 0.000122 0.011 0.0457 -0.178
Radioactive waste disposed (RWD) kg 4.22E-03 5.62E-06 6.56E-06 1.43E-05 -9.89E-04
Components for re-use (CRU) kg 0 0 0 0 0
Materials for recycling (MFR) kg 0 0 0 1.62 0
Materials for energy recovery (MER) kg 0 0 0 0 0
Exported electrical energy (EEE) MJ 0 0 0.529 1.52 0
Exported thermal energy (EET) MJ 0 0 0.959 2.97 0
References
Standards EN 15804:2012+A2:2019+AC:2021, Sustainability of
construction works — Environmental Product Declarations —
EN 15804 Core rules for the product category of construction products.
EN 15804:2012+A1 2013, Sustainability of construction works ISO 14025
— Environmental Product Declarations — Core rules for the
product category of construction products. EN ISO 14025:2011, Environmental labels and declarations —
Type III environmental declarations — Principles and
EN 15804 procedures.
4 Environmental-Product Declaration - dormakaba - BEST HD8000
Further References ISO 9001
Title of the software/database Quality Management System: ISO 9001:2015
Title of the software/database. Addition to the title, version. ISO 14001
Place: Publisher, Date of publication [Access on access date]. Environmental Management System: ISO 14001:2015
IBU 2021 ISO 50001
Energy Management System: ISO 50001:2011 UL 10C
Institut Bauen und Umwelt e.V.: General Instructions for the
EPD programme of Institut Bauen und Umwelt e.V., Version UL 10C, Positive pressure fire tests of door assemblies
2.0, Berlin: Institut Bauen und Umwelt e.V., 2021
www.ibu-epd.com GaBi ts
ADA thinkstep AG, GaBi Software System and Database for Life
Americans with Disabilities Act 1990 Cycle Engineering (SP39). 1992-2019 Copyright thinkstep AG
ANSI/ICC A117.1 PCR Part A
ANSI/ICC A117.1 - 2009, Accessible and usable buildings and Institut Bauen und Umwelt e.V., Product Category Rules for
facilities Construction Products from the range of Environmental Product
Declarations of Institut Bauen und Umwelt (IBU), Part A:
ANSI/BHMA A156.4 Calculation Rules for the Life Cycle Assessment and
Requirements on the Background Report
ANSI/BHMA A156.4 - 2013, Door controls — Closers
Candidate List of REACH Regulation /1907/2006/EC (date:
16.01.2020) PCR Part B
ECHA PCR Guidance-Texts for Building-Related Products and
Services. From the range of Environmental Product
European Chemicals Agency Declarations of Institute Construction and Environment e.V.
(IBU). Part B: Requirements on the EPD for building hardware
EN 15804 products
EN 15804:2012-04 REACH
Sustainability of construction works - Environmental product Registration, Evaluation, Authorisation and Restriction
declarations - Core rules for the product category of
construction products of Chemicals (REACH), Regulation (EC) No 1907/2006
5 Environmental-Product Declaration - dormakaba - BEST HD8000
Publisher
Institut Bauen und Umwelt e.V. +49 (0)30 3087748- 0
Hegelplatz 1 info@ibu-epd.com
10117 Berlin www.ibu-epd.com
Germany
Programme holder
Institut Bauen und Umwelt e.V. +49 (0)30 3087748- 0
Hegelplatz 1 info@ibu-epd.com
10117 Berlin www.ibu-epd.com
Germany
Author of the Life Cycle Assessment
Sphera Solutions GmbH +49 711 341817-0
Hauptstraße 111- 113 info@sphera.com
70771 Leinfelden-Echterdingen www.sphera.com
Germany
Owner of the Declaration
dormakaba International Holding GmbH +49 2333 793-0
DORMA Platz 1 info.de@dormakaba.com
58256 Ennepetal www.dormakaba.com
Germany
6 Environmental-Product Declaration - dormakaba - BEST HD8000
