Environmental Product Declaration
as per ISO 14025 and EN 15804
Owner of the declaration: Unifloor B.V.
Publisher: Kiwa-Ecobility Experts
Programme operator: Kiwa-Ecobility Experts
Declaration number: EPD-Unifloor-259-EN
Issue date: 11.11.2022
Valid to: 11.11.2027
Jumpax® ME
This Environmental Product Declaration (EPD) is based on the life cycle assessment of the
Jumpax® ME flooring system from Unifloor B.V. .
1. General information
Unifloor B.V. Jumpax® ME
Programme operator: Owner of the declaration:
Kiwa-Ecobility Experts Unifloor B.V.
Voltastr. 5 Arnsbergstraat 4
13355 Berlin 7418 EZ Deventer
Germany Netherlands
Declaration number: Declared unit:
EPD-Unifloor-259-EN 1 m2 Floor system
Issue date: Valid until:
11.11.2022 11.11.2027
Scope: Product category rules:
This EPD is based on the life cycle assessment PCR A - Calculation rules for the LCA and re-
of the Jumpax® ME flooring system from Uni- quirements for the background report
floor B.V. . PCR B - Resilient, textile and laminate floor
The declaration holder is liable for the under- coverings - Environmental product declara-
lying information and evidence. Kiwa-Ecobil- tions - Product category rules; EN 16810:2017
ity Experts is not liable for manufacturer in-
formation, life cycle assessment data and evi- Verification:
dence. The CEN standard EN 15804:2012+A2:2019
serves as the core PCR.
Independent verification of the declaration
and data according to EN ISO 14025:2011-10.
☐internal ☒external
Frank Huppertz Julian Rickert
(Head of Kiwa-Ecobility Experts) (Third party verifier)
Prof. Dr Frank Heimbecher
(Chairman of the Independent Expert Committee of
Kiwa-Ecobility Experts)
Environmental Product Declaration: Unifloor B.V. - Jumpax® ME | Page 2
2. Product
2.1 Product description & application
With Jumpax® ME (Micro Screed), Unifloor fills the gap between its classic Jumpax® Classic MDF sub-
floor system and a traditional dry screed structure. The result is a two-layer element system with the
typical Jumpax installation of 30 cm overlap and a simple, fast and firm contact adhesive connection.
Simple formats that arrive on site without transport damage and are created on site to form a ready-
to-install floor system. The solution for renovation of wooden floors or loft conversions as well as new
construction.
A fast and perfect system floor for critical subfloors for design coverings, linoleum or parquet floors.
Jumpax® ME is the practical combination of stability, mass and best impact sound reduction. Jumpax®
products are characterised by Uniform format of 120 x 60 cm, always 2-layer load distribution layer,
interactive contact adhesive, simple uniform installation grid, processing without sawing, almost dust-
free processing, floating installation, extremely stable and fast.
2.2 Technical data
In Table 1 the technical specifications of Jumpax® ME are listed.
Environmental Product Declaration: Unifloor B.V. - Jumpax® ME | Page 3
Table 1 : Technical data for Jumpax® ME
Parameter Value Unit
Strength 20 / ± 0,2 mm
Format 600 x 1200 / ± 1 mm
Weight per m² 25 kg
Weight per unit (per bottom & top panels) 18 kg
Bulk density 640 kg/m³
Residual moisture 1-2 %
Swelling in thickness after 24 hours:
Water absorption max < 2 %
Fire class RTF (according to standard EN13501:2007):
System check A -
fl-s1
Thermal resistance R value (according to ISO 8302:1991 and EN 12667:2001) 0,06 m².K/W
Permissible individual load 1,0 kN
Permissible payload 1,5/2,0 kN/m2
Impact sound insulation (IS) on screed floor (according to ISO 10140-3 2010
standard) in combination with 8 mm Cocofloor:
System check 25 dB ΔL
w
Impact sound insulation (IS) on wooden ceiling (according to ISO 10140-3 2010
base 64 dB) in combination with 4 mm Cocofloor:
System check 14 dB ΔL
n
in combination with CV 3 mm 14 dB ΔL
n
in combination with design floor 3 mm 16 dB ΔL
n
in combination with linoleum 2.5 mm 14 dB ΔL
n
in combination with Click design floor Rigid 6 mm 17 dB ΔL
n
in combination with Nora 2 mm 14 dB ΔL
n
in combination with 2-layer parquet 18 mm 17 dB ΔL
n
Formaldehyde content E-1 -
FSC certified FSC C154437 -
ETA ETA 18/0723 -
2.3 Production
Jumpax® ME is manufactured by Unifloor in Deventer in the Netherlands (Arnsbergstraat 4, 7418 EZ
Deventer). In this process, the individual layers (plaster etc.) are joined together with glue and then
packed for transport to the place of use (see Figure 1).
Figure 1 : Process flow diagram
Environmental Product Declaration: Unifloor B.V. - Jumpax® ME | Page 4
2.4 Raw materials
The structure consists of a 10 mm fibre-reinforced REA gypsum cover board with contact adhesive on
the underside. The base board is a multi-layer structure made of 10 mm fibre-reinforced REA gypsum
board, impact sound insulation on the underside and contact adhesive on the top. The "soft spring"
for the impact sound insulation consists of coconut fibres bound with natural latex, 8 mm thick, total
thickness 28 mm. The plasterboards provide mass and stability, the natural coir underlay provides the
balance and sound absorption for the best impact sound.
The product does not contain any substances from the candidate list of substances of very high concern
for authorisation (SVHC).
2.5 Packaging
The packaging consists of a pallet for transport and a protective film that is removed from the adhesive
surfaces during installation.
2.6 Reference service life (RSL)
Since the use phase is not considered, no reference useful life is given.
2.7 Other information
Further information on the product can be found on the manufacturer's website (www.unifloor.info).
Environmental Product Declaration: Unifloor B.V. - Jumpax® ME | Page 5
3. LCA: Calculation rules
3.1 Declared unit
The declared unit for floor systems is according to "PCR B - Resilient, textile and laminate floor cover-
ings - Environmental product declarations - Product category rules; EN 16810:2017" 1 m2 .
Table 2: Declared unit
Parameter Value Unit
Declared unit 1 m2
Conversion factor to 1 kg 0,040 m2 /kg
3.2 System boundary
The EPD was prepared in accordance with DIN EN 15804 and takes into account the manufacturing
phase, the construction phase and the disposal phase as well as the credits and loads outside the sys-
tem boundaries. This corresponds to the modules A1 to A3, A4 and A5 as well as C1 to C4 and D. The
type of EPD is therefore "cradle to grave with options".
In this life cycle assessment according to ISO 14025, the following phases of the product life cycle were
considered:
- A1: Raw material extraction and processing
- A2: Transport to the manufacturer
- A3: Production
- A4: Transport to the customer
- A5: Installation
- C1: Deconstruction
- C2: Transport
- C3: Waste treatment
- C4: Landfill
- D: Reuse, recovery and recycling potential
For the declared life phases, all inputs (raw materials, intermediate products, energy and auxiliary ma-
terials) as well as the waste produced were considered.
3.3 Assumptions and estimates
For data protection reasons, the assumptions made and data used are only explained in the back-
ground report accompanying this EPD.
3.4 Period under review
All product- and process-specific data were collected for the operating year 2021 and are thus up-to-
date.
Environmental Product Declaration: Unifloor B.V. - Jumpax® ME | Page 6
3.5 Cut-off criteria
Potential environmental impacts were assigned to the material flows based on the Ecoinvent database
version 3.6. All flows contributing to more than 1 percent of the total mass, energy or environmental
impacts of the system were considered in the LCA. It can be assumed that the neglected processes
would have contributed less than 5 percent to the impact categories considered.
Other operating resources and the corresponding waste were not considered part of the product sys-
tem and accordingly not included in the balancing.
3.6 Data quality
To ensure the comparability of the results, only consistent background data from the Ecoinvent data-
base version 3.6 (2019) was used in the LCA (e.g. data sets on energy, transports, auxiliary and operat-
ing materials). The database is regularly checked and thus complies with the requirements of EN 15804
(background data not older than 10 years). Almost all consistent data sets contained in the Ecoinvent
database version 3.6 are documented and can be viewed in the online documentation.
The raw material data were converted into reference flows (input per declared unit).
The general rule was followed that specific data from specific production processes or average data
derived from specific processes must have priority in the calculation of an LCA. Data for processes over
which the manufacturer has no influence were assigned generic data.
The LCA calculation was carried out using Nibe's LCA & EPD tool R< THiNK.
3.7 Allocation
Specific information on allocations within the background data can be found in the documentation of
the Ecoinvent database version 3.6 datasets.
3.8 Comparability
In principle, a comparison or assessment of the environmental impact of different products is only
possible if they have been produced in accordance with EN 15804. For the assessment of comparabil-
ity, the following aspects in particular must be taken into account: PCR used, functional or declared
unit, geographical reference, definition of the system boundary, declared modules, data selection
(primary or secondary data, background database, data quality), scenarios used for use and disposal
phases and the life cycle inventory (data collection, calculation methods, allocations, validity period).
PCRs and general programme instructions of different EPDs programmes may differ. Comparability
must be checked. Further guidance can be found in EN 15804+A2 (5.3 Comparability of EPDs for con-
struction products) and ISO 14025 (6.7.2 Requirements for comparability).
3.9 Data collection
ISO 14044 section 4.3.2 was taken into account in the data collection.
The objective and the scope of the study were defined in consultation with Unifloor B.V. . The data
collection took place with the help of an Excel data collection template provided by Kiwa GmbH. The
collected data was checked by Kiwa GmbH, for example by critically questioning the assumptions made
by Unifloor B.V. . In this way, some errors (e.g. unit errors) could be corrected in cooperation with
Unifloor B.V. . Subsequently, the annual values were related to the declared unit of one square metre
with the help of corresponding calculations. In addition, suitable assumptions were made and esti-
mates carried out for the missing information and data.
Environmental Product Declaration: Unifloor B.V. - Jumpax® ME | Page 7
3.10 Calculation method
For the life cycle assessment, the calculation procedures described in ISO 14044 section 4.3.3 were
applied. The evaluation is carried out on the basis of the phases lying within the system boundaries
and the processes contained therein.
Environmental Product Declaration: Unifloor B.V. - Jumpax® ME | Page 8
4. LCA: Scenarios and additional technical information
For the transport to the construction site in module A4, a scenario with a distance of 286 km and the
environmental profile "market group for transport, freight, lorry, unspecified {GLO}" from Ecoinvent
3.6 was used.
No auxiliary or operating materials or energy were taken into account when installing the product in
module A5, as only human muscle power is required for the installation. There are no direct emissions
into the ambient air, soil or water. But there is packaging waste in the form of protective film, which is
removed from the adhesive surfaces, and a Euro pallet, which was used for transport. As a conservative
approach, an additional 3 % installation waste was assumed.
For disposal, a waste scenario for "MDF" based on the NMD waste scenario ID 36 from the Netherlands
was adapted and used for Germany. Here, 5 % landfilling and 95 % incineration were assumed. For the
distance to waste treatment, 100 km for landfilling and 150 km for incineration were used with "market
group for transport, freight, lorry, unspecified {GLO}" (from Ecoinvent 3.6). The energy saving (credit)
from incineration was adjusted for the German market. For the landfill loads, "99% Waste wood, un-
treated and 1% Waste paint {EU}| treatment of, sanitary landfill" was used and for the incineration
"Waste building wood, chrome preserved {CH}| treatment of, municipal incineration".
Environmental Product Declaration: Unifloor B.V. - Jumpax® ME | Page 9
5. LCA: Results
The following tables show the results of the life cycle assessment, more specifically for the environ-
mental impact indicators, resource consumption, output streams and waste categories. The results
presented here refer to the declared unit of 1 m2 Jumpax® ME.
The results of the environmental impact indicators ETP- fw, HTP-c, HTP-nc, SQP, ADP-f, ADP-mm and
WDP must be used with caution, as the uncertainties in these results are high or there is limited expe-
rience with the indicator.
The IRP impact category mainly addresses the potential effect of low dose ionising radiation on human
health in the nuclear fuel cycle. It does not consider effects due to possible nuclear accidents and oc-
cupational exposure, nor does it consider the disposal of radioactive waste in underground facilities.
Potential ionising radiation from soil, radon and some building materials is also not measured by this
indicator.
Environmental Product Declaration: Unifloor B.V. - Jumpax® ME | Page 10
Description of system boundary (X = module declared; MND = module not declared)
Construction Benefits and loads beyond the
Production stage Use stage End of life stage
process stage system boundaries
e
s e
y
lp p u s la ir e t a m w a R t r o p s n a r T n o it c u d o r P t r o p s n a r T n o it a lla t s n I e s U e c n a n e t n ia M r ia p e R t n e m e c a lp e R t n e m h s ib r u fe R
u
y g r e n e la n o it a r e p O
s
u
r e t a w la n o it a r e p O n o it c u r t s n o c e D t r o p s n a r T g n is s ee tc so a Wr p la s o p s iD e s u e R-, ,y r e v o c e R la it n e t o p g n ilc y c e R
A1 A2 A3 A4 A5 B1 B2 B3 B4 B5 B6 B7 C1 C2 C3 C4 D
X X X X X MND MND MND MND MND MND MND X X X X X
Environmental Product Declaration: Unifloor B.V. - Jumpax® ME | Page 11
Table 3: LCA results - environmental impact indicators: 1 m2 Jumpax® ME
Parameter Unit A1 A2 A3 A4 A5 C1 C2 C3 C4 D
AP mol H+-eq. 6,59E-02 1,93E-03 3,68E-03 8,30E-03 2,48E-03 0,00E+00 3,04E-03 7,84E-03 1,21E-04 -1,59E-03
GWP-total kg CO2-eq. -4,38E+00 3,33E-01 1,70E+00 1,43E+00 1,05E+00 0,00E+00 5,24E-01 3,65E+01 1,47E-01 -8,83E-01
GWP-b kg CO2-eq. -9,53E+00 1,54E-04 6,41E-01 6,60E-04 8,29E-01 0,00E+00 2,42E-04 3,62E+01 1,31E-01 -4,10E-02
GWP-f kg CO2-eq. 5,01E+00 3,33E-01 1,06E+00 1,43E+00 2,16E-01 0,00E+00 5,24E-01 2,29E-01 1,56E-02 -8,42E-01
GWP-luluc kg CO2-eq. 1,47E-01 1,22E-04 4,61E-03 5,24E-04 4,56E-03 0,00E+00 1,92E-04 6,27E-05 6,84E-06 -6,11E-04
ETP-fw CTUe 3,77E+02 4,48E+00 1,73E+01 1,92E+01 1,24E+01 0,00E+00 7,04E+00 6,81E+00 3,30E-01 -4,63E+00
PM Occurrence of diseases 5,02E-07 2,99E-08 2,66E-08 1,29E-07 2,01E-08 0,00E+00 4,71E-08 6,32E-08 2,29E-09 -5,66E-09
EP-m kg N-eq. 2,87E-02 6,80E-04 1,34E-03 2,92E-03 1,06E-03 0,00E+00 1,07E-03 3,64E-03 7,80E-05 -2,93E-04
EP-fw kg PO4-eq. 6,73E-03 3,36E-06 2,21E-04 1,44E-05 2,09E-04 0,00E+00 5,28E-06 4,69E-06 2,91E-07 -7,61E-05
EP-t mol N-eq. 2,36E-01 7,50E-03 1,26E-02 3,22E-02 9,31E-03 0,00E+00 1,18E-02 4,17E-02 4,47E-04 -4,31E-03
HTP-c CTUh 1,04E-08 1,45E-10 3,42E-09 6,24E-10 3,34E-09 0,00E+00 2,28E-10 9,69E-08 9,18E-12 -1,04E-10
HTP-nc CTUh -1,74E-07 4,90E-09 -7,76E-10 2,10E-08 -4,13E-09 0,00E+00 7,70E-09 2,38E-08 3,53E-10 -3,79E-09
IRP kBq U235-eq. 3,91E-01 2,10E-02 2,67E-02 9,04E-02 1,44E-02 0,00E+00 3,31E-02 6,06E-03 1,29E-03 -2,38E-02
SQP - 1,63E+02 4,35E+00 2,01E+01 1,87E+01 5,87E+00 0,00E+00 6,85E+00 8,09E-01 7,80E-01 -1,52E+00
ODP kg CFC11-eq. 5,63E-07 7,34E-08 1,17E-07 3,16E-07 2,72E-08 0,00E+00 1,16E-07 2,94E-08 4,31E-09 -6,79E-08
POCP kg NMVOC eq. 2,82E-02 2,14E-03 2,46E-03 9,20E-03 1,42E-03 0,00E+00 3,37E-03 1,09E-02 1,60E-04 -9,26E-04
ADP-f MJ 7,18E+01 5,02E+00 1,57E+01 2,16E+01 3,11E+00 0,00E+00 7,90E+00 2,33E+00 3,30E-01 -1,24E+01
ADP-mm kg Sb-eq. 1,57E-04 8,43E-06 7,27E-06 3,62E-05 5,64E-06 0,00E+00 1,33E-05 1,43E-06 1,49E-07 -1,56E-06
WDP m3 World eq. withdrawn 1,91E+01 1,80E-02 6,22E-01 7,72E-02 5,97E-01 0,00E+00 2,82E-02 8,19E-02 1,41E-02 -1,85E-02
AP = Acidification potential, accumulated exceedance; GWP-total = Global warming potential, total; GWP-b = Global warming potential, biogenic; GWP-f = Global warming
potential, fossil; GWP-luluc = Global warming potential, land use and land use change; ETP-fw = Ecotoxicity potential, freshwater; PM = Particulate matter emissions disease
Environmental Product Declaration: Unifloor B.V. - Jumpax® ME | Page 12
potential; EP-m = Eutrophication potential, fraction of nutrients reaching marine saltwater end compartment; EP-fw = Eutrophication potential, fraction of nutrients reaching
freshwater end compartment; EP-t = Eutrophication potential, accumulated potential; HTP-c = Human toxicity potential, cancer effects; HTP-nc = Human toxicity potential, non-
cancer effects; IRP = Ionizing radiation potential, human health; SQP = Soil quality potential; ODP = Depletion potential of the stratospheric ozone layer; POCP = Formation
potential of tropospheric ozone; ADP-f = Abiotic depletion potential for fossil resources; ADP-mm = Abiotic depletion potential for non-fossil resources, minerals and metals;
WDP = Water deprivation potential, deprivation-weighted water consumption
Environmental Product Declaration: Unifloor B.V. - Jumpax® ME | Page 13
Table 4: LCA results - resource consumption, output streams & waste categories: 1 m2 Jumpax® ME
Parameter Unit A1 A2 A3 A4 A5 C1 C2 C3 C4 D
PERE MJ 1,38E+02 6,28E-02 6,64E+00 2,70E-01 4,35E+00 0,00E+00 9,88E-02 1,09E-01 7,05E-03 -9,00E-01
PERM MJ 0,00E+00 0,00E+00 0,00E+00 0,00E+00 0,00E+00 0,00E+00 0,00E+00 0,00E+00 0,00E+00 -2,45E-03
PERT MJ 1,38E+02 6,28E-02 6,64E+00 2,70E-01 4,35E+00 0,00E+00 9,88E-02 1,08E-01 5,80E-03 -9,02E-01
PENRE MJ 6,04E+01 5,33E+00 1,67E+01 2,29E+01 2,85E+00 0,00E+00 8,38E+00 3,57E+00 3,56E-01 -1,35E+01
PENRM MJ 1,62E+01 0,00E+00 5,36E-01 0,00E+00 5,03E-01 0,00E+00 0,00E+00 0,00E+00 0,00E+00 -6,78E-05
PENRT MJ 7,66E+01 5,33E+00 1,72E+01 2,29E+01 3,32E+00 0,00E+00 8,38E+00 2,51E+00 3,50E-01 -1,35E+01
SM kg 0,00E+00 0,00E+00 0,00E+00 0,00E+00 0,00E+00 0,00E+00 0,00E+00 0,00E+00 0,00E+00 0,00E+00
RSF MJ 0,00E+00 0,00E+00 0,00E+00 0,00E+00 0,00E+00 0,00E+00 0,00E+00 0,00E+00 0,00E+00 0,00E+00
NRSF MJ 0,00E+00 0,00E+00 0,00E+00 0,00E+00 0,00E+00 0,00E+00 0,00E+00 0,00E+00 0,00E+00 0,00E+00
FW m3 6,75E-01 6,11E-04 2,36E-02 2,63E-03 2,14E-02 0,00E+00 9,62E-04 1,22E-02 3,44E-04 -2,94E-03
HWD kg 1,84E-04 1,27E-05 2,21E-05 5,47E-05 7,65E-06 0,00E+00 2,00E-05 1,49E-05 5,07E-07 -9,07E-06
NHWD kg 1,02E+00 3,18E-01 1,22E-01 1,37E+00 1,05E-01 0,00E+00 5,01E-01 1,32E+00 1,32E+00 -2,86E-02
RWD kg 3,38E-04 3,30E-05 2,78E-05 1,42E-04 1,38E-05 0,00E+00 5,18E-05 7,18E-06 1,96E-06 -3,11E-05
CRU kg 0,00E+00 0,00E+00 0,00E+00 0,00E+00 0,00E+00 0,00E+00 0,00E+00 0,00E+00 0,00E+00 0,00E+00
MFR kg 0,00E+00 0,00E+00 0,00E+00 0,00E+00 1,78E-04 0,00E+00 0,00E+00 0,00E+00 0,00E+00 0,00E+00
MER kg 0,00E+00 0,00E+00 0,00E+00 0,00E+00 0,00E+00 0,00E+00 0,00E+00 2,50E+01 0,00E+00 0,00E+00
EET MJ 0,00E+00 0,00E+00 -2,27E-01 0,00E+00 0,00E+00 0,00E+00 0,00E+00 0,00E+00 0,00E+00 -7,77E+00
EEE MJ 0,00E+00 0,00E+00 -1,43E-01 0,00E+00 0,00E+00 0,00E+00 0,00E+00 9,25E+00 0,00E+00 -4,91E+00
PERE = Use of renewable primary energy excluding renewable primary energy resources used as raw materials; PERM = Use of renewable primary energy resources used as raw
materials; PERT = Total use of renewable primary energy resources; PENRE = Use of non-renewable primary energy excluding non-renewable primary energy resources used as
raw materials; PENRM = Use of non-renewable primary energy resources used as raw materials; PENRT = Total use of non-renewable primary energy resources; SM = Use of
secondary material; RSF = Use of renewable secondary fuels; NRSF = Use of non-renewable secondary fuels; FW = Use of net fresh water; HWD = Hazardous waste disposed;
Environmental Product Declaration: Unifloor B.V. - Jumpax® ME | Page 14
NHWD = Non-hazardous waste disposed; RWD = Radioactive waste disposed; CRU = Components for re-use; MFR = Materials for recycling; MER = Materials for energy recovery;
EET = Exported energy, thermic; EEE = Exported energy, electric
Environmental Product Declaration: Unifloor B.V. - Jumpax® ME | Page 15
6. LCA: Interpretation
For easier understanding, the results are presented graphically in order to be able to see correlations
and connections between the data more clearly.
The following figure shows the shares of the different product life phases in the environmental im-
pacts.
WDP
ADP-mm
ADP-f
POCP
ODP
SQP
IRP
HTP-nc
HTP-c
EP-t
EP-fw
EP-m
PM
ETP-fw
GWP-luluc
GWP-f
GWP-b
GWP-total
AP
-80% -60% -40% -20% 0% 20% 40% 60% 80% 100%
A1 A2 A3 A4 A5 C1 C2 C3 C4 D
Figure 2: Shares of the product life phases in the environmental impacts for Jumpax® ME
As can be seen in the graph, raw material provision A1 dominates in the production phase in almost
all environmental impacts. Furthermore, it can be seen from the negative values that the credits out-
side the system boundaries in module D predominate.
For "Human toxicity potential, non-cancer effects (HTP-nc)", the sum of the negative values outweighs
the sum of the positive values. In addition, a comparatively high credit for GWP-biogen in module A1
of -9.53 kg was found. This is primarily due to the raw material used, "coconut fibres", with a GWP-
biogenic value of -8.468 kg CO2e/kg.
Environmental Product Declaration: Unifloor B.V. - Jumpax® ME | Page 16
7. References
Ecoinvent, 2019 Ecoinvent database version 3.6, 2019
EN 15804: EN 15804:2012+A2:2019: Sustainability of construction works - Environmental
product declarations - Basic rules for the product category construction prod-
ucts
ISO 14025: DIN EN ISO 14025:2011-10: Environmental labels and declarations - Type III
environmental declarations - Principles and procedures
ISO 14040: DIN EN ISO 14040:2006-10, Environmental management - Life cycle assess-
ment - Principles and framework; EN ISO 14040:2006
ISO 14044: DIN EN ISO 14044:2006-10, Environmental management - Life cycle assess-
ment - Requirements and guidelines; EN ISO 14040:2006
PCR A: General product category rules for building products from the EPD programme
of Ecobility Experts GmbH: Calculation rules for the LCA and requirements for
the background report
PCR B: Resilient, textile and laminate floor coverings - Environmental product decla-
rations - Product category rules; EN 16810:2017
R< THiNK, 2022 R< THiNK; Online LCA & EPD tool from Nibe; 2022
Environmental Product Declaration: Unifloor B.V. - Jumpax® ME | Page 17
Publisher:
Kiwa-Ecobility Experts Mail DE.Ecobility.Experts@
Voltastrasse 5 kiwa.com
13355 Berlin Web www.kiwa.com/de/de/the-
Germany mes/ecobility-experts/
Programme operator:
Kiwa-Ecobility Experts Mail DE.Ecobility.Experts@
Voltastrasse 5 kiwa.com
13355 Berlin Web www.kiwa.com/de/de/the-
Germany mes/ecobility-experts/
Author of the Life Cycle
Assessment: Tel +49 30 467761 43
Kiwa GmbH Mail DE.Nachhaltigkeit@kiwa.com
Voltastrasse 5 Web www.kiwa.com
13355 Berlin
Germany
Owner of the declaration:
Unifloor B.V. Tel +31 570 85 55 33
Arnsbergstraat 4 Mail info@unifloor.nl
7418 EZ Deventer Web www.unifloor.nl
Netherlands
Kiwa-Ecobility Experts is
established member of the
Environmental Product Declaration: Unifloor B.V. - Jumpax® ME | Page 18
