ENVIRONMENTAL PRODUCT DECLARATION
as per ISO 14025 and EN 15804+A2
Owner of the Declaration dormakaba International Holding GmbH
Publisher Institut Bauen und Umwelt e.V. (IBU)
Programme holder Institut Bauen und Umwelt e.V. (IBU)
Declaration number EPD-DOR-20220258-CBA2-EN
Issue date 19.10.2022
Valid to 18.10.2027
Remote reader 91 25
dormakaba
www.ibu-epd.com | https://epd-online.com
General Information
dormakaba Remote reader 91 25
Programme holder Owner of the declaration
IBU – Institut Bauen und Umwelt e.V. dormakaba International Holding GmbH
Hegelplatz 1 DORMA Platz 1
10117 Berlin 58256 Ennepetal
Germany Germany
Declaration number Declared product / declared unit
EPD-DOR-20220258-CBA2-EN 1 piece of the product: Remote reader 91 25
This declaration is based on the product category rules: Scope:
Electronic and physical Access Control Systems, 01.08.2021 This EPD refers to a specific product manufactured by dormakaba. The
(PCR checked and approved by the SVR) production site is located in Villingen-Schwenningen (Germany).
The data represents the year 2020.
Issue date The owner of the declaration shall be liable for the underlying information
and evidence; the IBU shall not be liable with respect to manufacturer
19.10.2022
information, life cycle assessment data and evidences.
The EPD was created according to the specifications of EN 15804+A2. In
Valid to
the following, the standard will be simplified as EN 15804.
18.10.2027
Verification
The standard EN 15804 serves as the core PCR
Independent verification of the declaration and data according to ISO
14025:2011
internally X externally
Dipl.-Ing. Hans Peters
(Chairman of Institut Bauen und Umwelt e.V.)
Florian Pronold Dr.-Ing. Wolfram Trinius,
(Managing Director Institut Bauen und Umwelt e.V.) (Independent verifier)
1 Environmental Product Declaration - dormakaba - Remote reader 91 25
Product
Interfaces
Product description/Product definition • 2 coaxial connections for registration units
The dormakaba remote reader 91 25 is a powerful access • RS-485: Connection to host system
control unit which monitors many access points. Thanks to an • 4 binary inputs: max. 5 V DC
extensive range of operating modes, the dormakaba remote • 3 relay outputs: max. 34 V DC/60 W, 27 V AC/60 VA
reader 91 25 supports all commonly implemented door • 1 tamper switch
configurations. Two registration units can be connected to one • 2 RS-232 interfaces
remote reader, meaning one reader is sufficient to achieve an
in/out configuration. Modularly extendible digital inputs and Supported RFID technologies
outputs enable the monitoring of frame and deadbolt contacts •LEGIC (advant & prime)
in complex door configurations, as well as the setting off •MIFARE (DESFire & Classic)
alarms. For the placing on the market in the European
Union/European Free Trade Association (EU/EFTA) (with the Power supply
exception of Switzerland) the following legal provisions apply: 12 - 27 V AC 50/60 Hz or 10 - 34 V DC
• Restriction of Hazardous Substances (RoHS) Class of protection as per EN 60529:IP20.
• Radio Equipment Directive (RED)
The CE-marking takes into account the proof of conformity with The product is not harmonised in accordance with the
the respective harmonized standards based on the legal Construction Product Regulations (CPR) but in accordance with
provisions above. For the application and use the respective other provisions for harmonisation of the EU. Compliance with
national provisions apply. the European Union Directive and technical specifications:
• EN 62368-1
Application
• EN 301489-1 V2.1.1
The reader is particularly suitable for demanding access points, • EN 301489-3 V2.1.0
such as turnstiles and personal interlocks, where a high level of • EN 300330 V2.1.1
security is required. The remote reader 91 25 is available in • EN 50364
different versions, depending on type of function, and supports The product is subject to CE marking according to the relevant
selected devices from other manufacturers, as well as harmonization legislation.
dormakaba registration units. In addition, the product also conforms to the following
standards:
Areas of application:
• UL62368-1
• Turnstiles • CAN/CSA-22.2 No.
• Personal interlocks 62368-1
• External gates and gateways
• Automatic doors Base materials/Ancillary materials
• Lifts The major material compositions including the packaging of the
• Car park barriers product are listed below:
• Entrance areas
Name Value Unit
• Motor locks
Electronics 45 %
Technical Data Plastics 26 %
The remote reader 91 25 has the following technical properties: Paper 29 %
Name Value Unit
The product includes partial articles which contain substances
Operating Temperature 0 - 50 °C listed in the Candidate List of REACH Regulation
Operating Humidity 0 - 95 % 1907/2006/EC (date: 17.01.2022) exceeding 0.1 percentage by
Width Dimension 125 mm mass in the alloy: no
The Candidate List can be found on the ECHA website
Height Dimension 102 mm
address: https:echa.europa.eu/de/home.
Depth Dimension 45 mm
Weight (without packaging) 0,176 kg Reference service life
Weight (with packaging) 0,249 kg The reference service life of the dormakaba remote reader 91
Power consumption "idle mode" 2 W 25 is estimated to be 15 years. This number is based on the
support and service life and is not an estimated lifetime.
Power consumption "on mode" 5 W
LCA: Calculation rules
Declared Unit
The declared unit is 1 piece of the product: Remote reader 91 System boundary
25. The type of EPD is: cradle to gate with options, modules C1–
Name Value Unit C4, and module D (A1–A3 + C + D and additional modules: A4
+ A5 + B6)
Declared unit 1 pce.
Product weight including packaging 0,249 kg
Production - Module A1-A3
The product stage includes:
— A1, raw material extraction, processing and mechanical
2 Environmental Product Declaration - dormakaba - Remote reader 91 25
treatments, processing of secondary material input (e.g. — C2, transport to waste processing;
recycling processes), — C3, waste processing for reuse, recovery and/or recycling;
— A2, transport to the manufacturer, — C4, disposal; including provision and all transport, provision
— A3, manufacturing and assembly including provision of all of all materials, products and related energy and water use.
materials, products and energy, as well as waste processing up
to the end-of waste state. Module D (Benefits and loads beyond the system boundary)
includes:
Construction stage - Modules A4-A5 — D, recycling potentials, expressed as net impacts and
The construction process stage includes: benefits.
— A4, transport to the building site;
— A5, installation into the building;including provision of all Geographic Representativeness
materials, products and energy, as well as waste processing up Land or region, in which the declared product system is
to the end-of-waste state or disposal of final residues during the manufactured, used or handled at the end of the product´s
construction process stage. lifespan: Germany
Use stage - Module B6
Comparability
The use stage related to the operation of the building includes:
Basically, a comparison or an evaluation of EPD data is only
— B6, operational energy use
possible if all the data sets to be compared were created
according to EN 15804 and the building context, respectively
End-of-life stage– Modules C1-C4 and D
the product-specific characteristics of performance, are taken
The end-of-life stage includes:
into account. Background database: GaBi, SP40.
— C1, de-construction, demolition:
LCA: Scenarios and additional technical information
Operational energy use (B6) and Operational water use
Characteristic product properties of biogenic carbon
(B7)
Information on describing the biogenic Carbon Content at The use stage is declared for 12 years.
factory gate
Name Value Unit
Name ValueUnit
Energy consumption for 1 year 13,51 kWh
Biogenic carbon content in accompanying kg
0.03 on mode per day 4 h
packaging C
idle mode 20 h
Note: 1 kg of biogenic carbon is equivalent to 44/12 kg of CO .
2 on mode power 5 W
idle mode 2 W
Days per year in use 365 days
The following technical scenario information is required for the
declared modules.
End of life (C1-C4)
Transport to the building site (A4) C1: The product dismantling from the building is done manually
Name Value Unit without environmental burden.
Litres of fuel per 1 kg (truck) 0.002766 l/100km Name Value Unit
Transport distance (truck) 100 km Collected separately waste type 0.177 kg
Capacity utilisation (including empty runs) 55 % Recycling 0.112 kg
Energy recovery 0.064 kg
Installation into the building (A5)
Final deposition 0,0005 kg
Name Value Unit
Transportation to Waste 50 km
Waste Packaging (paper) 0,072 kg
Region for end of life: Global
Reference service life
Name Value Unit Reuse, recovery and/or recycling potentials (D), relevant
scenario information
Life Span according to the manufacturer 12 a
Collection rate is 100%.
3 Environmental Product Declaration - dormakaba - Remote reader 91 25
LCA: Results
DESCRIPTION OF THE SYSTEM BOUNDARY (X = INCLUDED IN LCA; MND = MODULE OR INDICATOR NOT DECLARED; MNR
= MODULE NOT RELEVANT)
Benefits and
Construction loads beyond
Product stage Use stage End of life stage
process stage the system
boundaries
la ire ta m w a Ry lp p u s tro p s n a rT g n iru tc a fu n a M e h t m o rf tro p s n a rTe tis e h t o t e ta g y lb m e s s A e s U e c n a n e tn ia M ria p e R tn e m e c a lp e R tn e m h s ib ru fe R y g re n e la n o ita re p Oe s u re ta w la n o ita re p Oe s u n o itc u rts n o c -e Dn o itilo m e d tro p s n a rT g n is s e c o rp e ts a W la s o p s iD -e s u e R-y re v o c e R-g n ilc y c e Rla itn e to p
A1 A2 A3 A4 A5 B1 B2 B3 B4 B5 B6 B7 C1 C2 C3 C4 D
X X X X X MND MND MNR MNR MNR X MND X X X X X
RESULTS OF THE LCA - ENVIRONMENTAL IMPACT according to EN 15804+A2: 1 piece Remote reader 91 25
Parameter Unit A1-A3 A4 A5 B6 C1 C2 C3 C4 D
GWP-total kg CO 2 eq 4.18E+00 2E-03 1.02E-01 9.96E+01 0 6.21E-04 1.63E-01 7.63E-06 -1.32E-01
GWP-fossil kg CO 2 eq 4.27E+00 2E-03 3E-03 9.94E+01 0 5.93E-04 1.63E-01 7.58E-06 -1.32E-01
GWP-biogenic kg CO 2 eq -9.76E-02 9.62E-05 9.9E-02 1.09E-01 0 2.74E-05 3.8E-06 2.59E-08 -2.49E-04
GWP-luluc kg CO 2 eq 4.15E-03 4.95E-08 1.68E-06 1.37E-01 0 1.41E-08 9.22E-06 2.18E-08 -1.26E-04
ODP kg CFC11 eq 3.58E-10 2.2E-19 1.84E-17 1.05E-12 0 6.26E-20 8.23E-17 2.81E-20 -1.21E-15
AP mol H+ eq 3.22E-02 2.08E-06 2.86E-05 5.89E-01 0 5.94E-07 2.91E-05 5.44E-08 -8.56E-04
EP-freshwater kg P eq 2.13E-05 4.46E-10 3.59E-09 1.39E-04 0 1.27E-10 1.31E-08 1.3E-11 -1.52E-07
EP-marine kg N eq 5.07E-03 6.63E-07 1.03E-05 8.8E-02 0 1.89E-07 6.55E-06 1.4E-08 -1.07E-04
EP-terrestrial mol N eq 5.96E-02 7.37E-06 1.29E-04 9.55E-01 0 2.1E-06 1.32E-04 1.54E-07 -1E-03
kg NMVOC
POCP 1.62E-02 1.87E-06 2.73E-05 2.59E-01 0 5.34E-07 1.81E-05 4.24E-08 -3.3E-04
eq
ADPE kg Sb eq 2E-03 6.24E-11 2.9E-10 1.51E-05 0 1.78E-11 1.13E-09 6.81E-13 -4.19E-05
ADPF MJ 5.18E+01 3E-02 3.2E-02 1.33E+03 0 8E-03 7.6E-02 9.95E-05 -2.7E+00
m3 world eq
WDP 8.54E-01 4.08E-06 1.3E-02 2.07E+01 0 1.16E-06 1.7E-02 7.95E-07 -1.7E-02
deprived
GWP = Global warming potential; ODP = Depletion potential of the stratospheric ozone layer; AP = Acidification potential of land and water; EP =
Eutrophication potential; POCP = Formation potential of tropospheric ozone photochemical oxidants; ADPE = Abiotic depletion potential for non-fossil
resources; ADPF = Abiotic depletion potential for fossil resources; WDP = Water (user) deprivation potential)
RESULTS OF THE LCA - INDICATORS TO DESCRIBE RESOURCE USE according to EN 15804+A2: 1 piece Remote reader 91
25
Parameter Unit A1-A3 A4 A5 B6 C1 C2 C3 C4 D
PERE MJ 1.19E+01 9.31E-05 8.69E-01 4.19E+02 0 2.65E-05 2.6E-02 1.3E-05 -4.39E-01
PERM MJ 8.69E-01 0 -8.63E-01 0 0 0 -6E-03 0 0
PERT MJ 1.28E+01 9.31E-05 6E-03 4.19E+02 0 2.65E-05 2E-02 1.3E-05 -4.39E-01
PENRE MJ 4.88E+01 3E-02 3.2E-02 1.33E+03 0 8E-03 3.07E+00 9.96E-05 -2.7E+00
PENRM MJ 2.99E+00 0 0 0 0 0 -2.99E+00 0 0
PENRT MJ 5.18E+01 3E-02 3.2E-02 1.33E+03 0 8E-03 7.6E-02 9.96E-05 -2.7E+00
SM kg 0 0 0 0 0 0 0 0 0
RSF MJ 0 0 0 0 0 0 0 0 0
NRSF MJ 0 0 0 0 0 0 0 0 0
FW m3 2.3E-02 1.67E-07 2.98E-04 6.77E-01 0 4.76E-08 3.99E-04 2.51E-08 -5.28E-04
PERE = Use of renewable primary energy excluding renewable primary energy resources used as raw materials; PERM = Use of renewable primary
energy resources used as raw materials; PERT = Total use of renewable primary energy resources; PENRE = Use of non-renewable primary energy
excluding non-renewable primary energy resources used as raw materials; PENRM = Use of non-renewable primary energy resources used as raw
materials; PENRT = Total use of non-renewable primary energy resources; SM = Use of secondary material; RSF = Use of renewable secondary fuels;
NRSF = Use of non-renewable secondary fuels; FW = Use of net fresh water
RESULTS OF THE LCA – WASTE CATEGORIES AND OUTPUT FLOWS according to EN 15804+A2:
1 piece Remote reader 91 25
Parameter Unit A1-A3 A4 A5 B6 C1 C2 C3 C4 D
HWD kg 2.85E-06 2.87E-12 4.74E-11 6.75E-07 0 8.17E-13 2.88E-10 1.52E-12 -3.36E-09
NHWD kg 1E-01 3.02E-06 3E-03 7.36E-01 0 8.61E-07 1.7E-02 5.01E-04 4E-03
RWD kg 1.03E-03 3.17E-08 1.69E-06 1.13E-01 0 9.04E-09 2.81E-06 1.13E-09 -1.39E-04
CRU kg 0 0 0 0 0 0 0 0 0
MFR kg 0 0 0 0 0 0 7.7E-02 0 0
MER kg 0 0 0 0 0 0 0 0 0
EEE MJ 0 0 1.54E-01 0 0 0 0 0 0
EET MJ 0 0 2.8E-01 0 0 0 0 0 0
4 Environmental Product Declaration - dormakaba - Remote reader 91 25
HWD = Hazardous waste disposed; NHWD = Non-hazardous waste disposed; RWD = Radioactive waste disposed; CRU = Components for re-use;
MFR = Materials for recycling; MER = Materials for energy recovery; EEE = Exported electrical energy; EET = Exported thermal energy
RESULTS OF THE LCA – additional impact categories according to EN 15804+A2-optional:
1 piece Remote reader 91 25
Parameter Unit A1-A3 A4 A5 B6 C1 C2 C3 C4 D
Disease
PM 2.9E-07 1.1E-11 1.58E-10 9.05E-06 0 3.12E-12 3.71E-10 6.74E-13 -7.05E-09
incidence
IR kBq U235 eq 9.9E-02 4.53E-06 2.62E-04 1.78E+01 0 1.29E-06 2.53E-04 1.17E-07 -2.2E-02
ETP-fw CTUe 1.97E+01 2.1E-02 1.5E-02 4.23E+02 0 6E-03 2.8E-02 5.69E-05 -6.35E-01
HTP-c CTUh 1.16E-09 3.94E-13 8.08E-13 1.98E-08 0 1.12E-13 2.46E-12 8.43E-15 -3.38E-11
HTP-nc CTUh 5.46E-08 1.68E-11 3.5E-11 8.28E-07 0 4.8E-12 2.49E-10 9.29E-13 -1.99E-09
SQP SQP 1.89E+01 7.59E-05 9E-03 3.19E+02 0 2.16E-05 2.3E-02 2.08E-05 -4.98E-01
PM = Potential incidence of disease due to PM emissions; IR = Potential Human exposure efficiency relative to U235; ETP-fw = Potential comparative
Toxic Unit for ecosystems; HTP-c = Potential comparative Toxic Unit for humans (cancerogenic); HTP-nc = Potential comparative Toxic Unit for humans
(not cancerogenic); SQP = Potential soil quality index
Disclaimer 1 – for the indicator IRP This impact category deals mainly with the eventual impact of low dose ionizing radiation on human
health of the nuclear fuel cycle. It does not consider effects due to possible nuclear accidents, occupational exposure nor due to
radioactive waste disposal in underground facilities. Potential ionizing radiation from the soil, from radon and from some construction
materials is also not measured by this indicator.
Disclaimer 2 – for the indicators ADPE, ADPF, WDP, ETP-fw, HTP-c, HTP-nc, SQP
The results of this environmental impact indicator shall be used with care as the uncertainties on these results are high or as there is
limited experience with the indicator. This EPD was created using a software tool.
References
CAN/CSA-22.2 No. 62368-1
CAN/CSA-22.2 No. 62368-1:2014, Audio/video, information and ISO 14025
communication technologyequipment — Part 1: Safety DIN EN ISO 14025:2011-10, Environmental labels and
requirements declarations — Type III environmental declarations —
Principles and procedures
EN 15804
EN 15804+A2:2019+AC:2021, Sustainability of construction Radio Equipment Directive (RED)
works — Environmental Product Declarations — Core rules for Directive 2014/53/EU of the European Parliament and of the
the product category of construction products Council of 16 April 2014 on the harmonisation of the laws of the
Member States relating to the making available on the market
EN 300330 V2.1.1 of radio equipment and repealing Directive 1999/5/EC
Short Range Devices (SRD) - Radio equipment in the
frequency range 9 kHz to 25 MHz and inductive loop systems in Registration, Evaluation, Authorisation and Restriction of
the frequency range 9 kHz to 30 MHz - Harmonised Standard Chemicals (REACH)
covering the essential requirements of article 3.2 of the Regulation (EC) No 1907/2006 of the European Parliament and
Directive 2014/53/EU of the Council on the Registration, Evaluation, Authorisation
and Restriction of Chemicals (REACH)
EN 301489-1 V2.2.1
ElectroMagnetic Compatibility (EMC) standard for radio Restriction of Hazardous Substances (RoHS)
equipment and services - Part 1: Common technical Directive on the restriction of the use of certain hazardous
requirements - Harmonised Standard covering the essential substances in electrical and electronic equipment (RoHS),
requirements of article 3.1(b) of Directive 2014/53/EU and the Directive (EU) No 2011/65
essential requirements of article 6 of Directive 2014/30/EU
UL 62368-1
EN 301489-3 V2.1.1 UL 62368-1:2014, Standard for Audio/video, information and
ElectroMagnetic Compatibility (EMC) standard for radio communication technology equipment - Part 1: Safety
equipment and services - Part 3: Specific conditions for Short- requirements
Range Devices (SRD) operating on frequencies between 9 kHz
and 246 GHz - Harmonised standard covering the essential Further References
requirements of article 3.1(b) of Directive 2014/53/EU
IBU
EN 50364 Institut Bauen und Umwelt e.V.: General Instructions for the
EN 50364:2010, Limitation of human exposure to EPDs programme of Institut Bauen und Umwelt e.V. Version
electromagnetic fields from devices operating in the frequency 2.0., Berlin: Institut Bauen und Umwelt e.V., 2021. www.ibu-
range 0 Hz to 300 GHz, used in Electronic Article Surveillance epd.com
(EAS), Radio Frequency Identification (RFID) and similar
applications GaBi ts software
Sphera Solutions GmbH
EN 62368-1 Gabi Software System and Database for Life Cycle Engineering
EN 62368-1:2014, Audio/video, information and communication 1992-2020 Version 10.0.0.71 University of Stuttgart Leinfelden-
technology equipment - Part 1: Safety requirements Echterdingen
5 Environmental Product Declaration - dormakaba - Remote reader 91 25
GaBi ts documentation
GaBi life cycle inventory data documentation (https://www.gabi-
software.com/support/gabi/gabi-database-2020-lci-
documentation/)
LCA-tool dormakaba
LCA tool, IBU-DOR-202102-LT1-EN.
Developed by Sphera Solutions GmbH
PCR Part A
PCR – Part A:
Calculation Rules for the Life Cycle As-sessment and
Requirements on the Project Re-port according to EN
15804+A2:2019, Version 1.0, Institut Bauen und Umwelt e.V.,
www.ibu-epd.com
PCR Part B
PCR – Part B: Requirements on the EPD for Building Hardware
product, version 1.3, Institut Bauen und Umwelt e.V., www.ibu-
epd.com, 2019
6 Environmental Product Declaration - dormakaba - Remote reader 91 25
Publisher
Institut Bauen und Umwelt e.V. +49 (0)30 3087748- 0
Hegelplatz 1 info@ibu-epd.com
10117 Berlin www.ibu-epd.com
Germany
Programme holder
Institut Bauen und Umwelt e.V. +49 (0)30 3087748- 0
Hegelplatz 1 info@ibu-epd.com
10117 Berlin www.ibu-epd.com
Germany
Author of the Life Cycle Assessment
Sphera Solutions GmbH +49 711 341817-0
Hauptstraße 111- 113 info@sphera.com
70771 Leinfelden-Echterdingen www.sphera.com
Germany
Owner of the Declaration
dormakaba International Holding GmbH +49 2333 793-0
DORMA Platz 1 info.de@dormakaba.com
58256 Ennepetal www.dormakaba.com
Germany
7 Environmental Product Declaration - dormakaba - Remote reader 91 25
