ENVIRONMENTAL PRODUCT DECLARATION
as per ISO 14025 and EN 15804+A1
Owner of the Declaration ArcelorMittal Brasil
Programme holder Institut Bauen und Umwelt e.V. (IBU)
Publisher Institut Bauen und Umwelt e.V. (IBU)
Declaration number EPD-ARC-20190175-CBC2-EN
Issue date 09.03.2020
Valid to 08.03.2025
Hot Dip Galvanized Steel with Pure Zinc Coating
ArcelorMittal Brasil
www.ibu-epd.com | https://epd-online.com
Umwelt Produktdeklaration Name des Herstellers – Name des Produkts
General Information
ArcelorMittal Brasil Hot dip galvanized steel with pure zinc
coating
Programme holder Owner of the declaration
IBU – Institut Bauen und Umwelt e.V. ArcelorMittal Brasil
Panoramastr. 1 Av. Carandaí, 1115
10178 Berlin 30130-915 - Belo Horizonte - MG
Germany Brazil
Declaration number Declared product / declared unit
EPD-ARC-20190175-CBC2-EN 1 metric ton of Hot Dip Galvanized produced by
ArcelorMittal in Brazil
This declaration is based on the product Scope:
category rules: This declaration and its LCA study are relevant to Hot
Structural steels, 07.2014 Dip Galvanized steel manufactured by ArcelorMittal
(PCR checked and approved by the SVR) Brasil, representing 100% of the production in 2017.
Issue date The owner of the declaration shall be liable for the
09.03.2020 underlying information and evidence; the IBU shall not
be liable with respect to manufacturer information, life
cycle assessment data and evidences.
Valid to
The EPD was created according to the specifications
08.03.2025
of EN 15804+A1. In the following, the standard will be
simplified as EN 15804.
Verification
The standard EN 15804 serves as the core PCR
Independent verification of the declaration and data
according to ISO 14025:2010
Dipl. Ing. Hans Peters internally x externally
(chairman of Institut Bauen und Umwelt e.V.)
Dr. Alexander Röder Dr.-Ing. Wolfram Trinius
(Managing Director Institut Bauen und Umwelt e.V.)) (Independent verifier appointed by SVR)
Product
Product description/Product definition acoustic panels for roofs and facades, flashings and
gutters, cable trays, conduits and components for
Zinc coated steel is obtained through the hot-dip electrical installations, silos, in addition to online
galvanizing process (where the steel is bathed in applications and in the agricultural and machinery
melted zinc); this coating produces high surface segments, etc.
quality, corrosion resistant and malleable steel. The Additional applications are also possible in other
result is a strip that is proper for the manufacturing of market segments.
both exposed and non-exposed parts for a variety of
applications. The single operation production process Technical Data
occurs in ArcelorMittal Vega which can produce coated
coils in thickness varying from 0.40 to 2.3mm and Hot dip galvanised products offer excellent corrosion
several widths depending on the steel grade. resistance combined with very good forming
properties.
For the use and application of the product the
respective national provisions at the place of use The coating process can apply various thickness of the
apply. zinc layer, up to 450 g/m² (total of both sides). Specific
mechanical properties are defined for each steel grade
used as substrate.
Application
Name Value Unit
Zinc coated steels are delivered in wide coils and used Density 7825 kg/m³
in a very large range of applications for industrial Thermal conductivity 48 W/(mK)
markets and for construction markets (indoor and Modulus of elasticity 210000 N/mm²
outdoor use). Some of the most common applications Coefficient of thermal expansion 12 10-6K-1
are: building structures, profiles for light steel framing, Melting point 1536 °C
profiles for drywall, steel deck, tiles and thermo-
2 Environmental Product Declaration ArcelorMittal Brasil – Hot Dip Galvanized
Performance data of the product with respect to its Base materials/Ancillary materials
characteristics in accordance with the relevant
technical provision (no CE-marking). The base material of zinc-coated steel is iron. Alloying
elements are added on the form of ferroalloys or
Delivery Status metals. The metallic coating includes only zinc.
Detailed information about mechanical properties and
The specifications of this declared product are given in coatings are available at:
NBR 7008-2:2012 (Steel-coated coils and plates with https://brasil.arcelormittal.com/produtos-
zinc or zinc-iron alloy by hot-dip continuous process solucoes/catalogos
immersion Part 2: Commercial quality steel stamping),
NBR 7008-3:2012 (Steel-coated coils and plates with Reference service life
zinc or zinc-iron alloy by hot-dip continuous process
immersion Part 3: Structural steels). The quantities Reference service life is not relevant due to cradle-to-
may vary according to the intended application. It can gate with options (C3 and D) boundary conditions
be delivered to the point of placement in a variety of
ways: wide coils, slit coils or sheets ready to be
processed through various technologies: bending, roll
forming, drawing, welding, perforating & cutting,
painting, etc.
LCA: Calculation rules
Declared Unit  Recycling of production/manufacturing scrap.
Steel scrap is assumed to reach the end-of-
The declared unit refers to the functional unit of 1
waste status once is shredded and sorted,
metric ton of double-sided zinc-coated steel as
thus becomes an input to the product system
specified in Part B requirements on the EPD for
in the inventory.
Structural Steel.
Declared unit Module C3 takes into account the sorting and
Name Value Unit shredding of after-use steel, as well as the non-
Declared unit 1 t recovered scrap due to sorting efficiency which is
Thickness (of sheet) 1 mm landfilled. A conservative value of 2% landfill is
Coating density 7.1 g/cm³ considered.
Conversion factor to 1 kg 0.001 -
Module D refers to the net benefits and loads of the
net flow leaving the product system.
System boundary Data Quality
The study is performed from ‘cradle-to-gate’ + module The life cycle inventory data used in this study comply
C3 and module D (cradle to gate – with Options). The with the quality requirements set out in ISO 14044.
following life cycle stages are considered:
 Product stage All relevant background datasets are taken from GaBI
 End-of-life through Waste processing ts Software database - Service Pack 37 and comprise
the year 2018. Such database contains consistent and
 Benefits and loads beyond the product
documented datasets which can be viewed in the
system boundary
online GaBI ts documentation.
Modules A1-A3 include the following: Regarding foreground data, this study is based on a
 The provision of resources, additives and high quality of primary data for the year 2017, collected
by ArcelorMittal.
energy;
 Transport of resources additives to the
Comparability
production site Basically, a comparison or an evaluation of EPD data
 Production processes on site including is only possible if all the data sets to be compared
energy, production of additives, disposal of were created according to EN 15804 and the building
production residues, and consideration of context, respectively the product-specific
characteristics of performance, are taken into account.
related emissions;
.
LCA: Scenarios and additional technical information
End of life (C3)
3 Environmental Product Declaration ArcelorMittal Brasil – Hot Dip Galvanized
Due to the absence of official national references and
recommendation of the Brazilian context, Recycling
and Reuse rates adopted for this EPD were defined
according to the recommendations of European
Commission Technical Steel Research for “Other
steel”: 99% (Recycling and Reuse) and 1% (Landfill).
Such assumptions are similar to current practices and
rates in the Brazilian market, which would not result in
visible changes of the EPD results.
Name Value Unit
Landfilling 10 kg
Reuse, recovery and/or recycling potentials (D),
relevant scenario information
45 kg scrap is used in the manufacturing of 1 ton of
HDG steel. After use, 990 kg steel is recycled.
The potential environmental benefit calculated for the
end-of-life stage (module D) is based on the net
amount of scrap in the system: 990 – 45 = 945 kg. The
system net output carries a potential credit, thus
module D shows an environmental benefit.
Name Value Unit
Reuse 11 %
Recycling 88 %
Landfill 1 %
4 Environmental Product Declaration ArcelorMittal Brasil – Hot Dip Galvanized
LCA: Results
DESCRIPTION OF THE SYSTEM BOUNDARY (X = INCLUDED IN LCA; MND = MODULE NOT DECLARED;
MNR = MODULE NOT RELEVANT)
BENEFITS AND
CONSTRUCTI LOADS
PRODUCT STAGE ON PROCESS USE STAGE END OF LIFE STAGE BEYOND THE
STAGE SYSTEM
BOUNDARIES
5 Environmental Product Declaration ArcelorMittal Brasil – Hot Dip Galvanized
lairetam
waR
ylppus tropsnarT
gnirutcafunaM
eht
morf
tropsnarT
etis
eht
ot
etag
ylbmessA esU
ecnanetniaM
riapeR
tnemecalpeR tnemhsibrufeR
ygrene
lanoitarepO esu
retaw
lanoitarepO esu
noitcurtsnoc-eD
noitilomed tropsnarT
gnissecorp
etsaW
lasopsiD -esueR -yrevoceR -gnilcyceR laitnetop
A1 A2 A3 A4 A5 B1 B2 B3 B4 B5 B6 B7 C1 C2 C3 C4 D
X X X MND MND MND MND MNR MNR MNR MND MND MND MND X MND X
RESULTS OF THE LCA - ENVIRONMENTAL IMPACT according to EN 15804+A1: 1 t Hot Dip Galvanized
Parameter Unit A1-A3 C3 D
Global warming potential [kg CO2-Eq.] 2.66E+3 2.54E+1 -1.52E+3
Depletion potential of the stratospheric ozone layer [kg CFC11-Eq.] 2.44E-5 3.14E-6 8.47E-6
Acidification potential of land and water [kg SO2-Eq.] 1.33E+1 2.30E-1 -2.99E+0
Eutrophication potential [kg (PO4)3--Eq.] 1.68E+0 1.04E-1 -2.22E-1
Formation potential of tropospheric ozone photochemical
[kg ethene-Eq.] 1.35E+0 1.77E-2 -7.02E-1
oxidants
Abiotic depletion potential for non-fossil resources [kg Sb-Eq.] 2.53E-2 4.61E-4 -4.66E-3
Abiotic depletion potential for fossil resources [MJ] 2.54E+4 3.55E+2 -1.47E+4
RESULTS OF THE LCA - RESOURCE USE according to EN 15804+A1: 1 t Hot Dip Galvanized
Parameter Unit A1-A3 C3 D
Renewable primary energy as energy carrier [MJ] 1.98E+3 5.40E+1 9.77E+2
Renewable primary energy resources as material utilization [MJ] 0.00E+0 0.00E+0 0.00E+0
Total use of renewable primary energy resources [MJ] 1.98E+3 5.40E+1 9.77E+2
Non-renewable primary energy as energy carrier [MJ] 2.60E+4 4.06E+2 -1.42E+4
Non-renewable primary energy as material utilization [MJ] 0.00E+0 0.00E+0 0.00E+0
Total use of non-renewable primary energy resources [MJ] 2.60E+4 4.06E+2 -1.42E+4
Use of secondary material [kg] 0.00E+0 0.00E+0 9.45E+2
Use of renewable secondary fuels [MJ] -2.15E-30 0.00E+0 0.00E+0
Use of non-renewable secondary fuels [MJ] -2.56E-29 0.00E+0 0.00E+0
Use of net fresh water [m³] 7.25E+0 1.83E-1 2.04E+0
RESULTS OF THE LCA – OUTPUT FLOWS AND WASTE CATEGORIES according to EN 15804+A1:
1 t Hot Dip Galvanized
Parameter Unit A1-A3 C3 D
Hazardous waste disposed [kg] 2.93E-4 3.84E-8 -9.93E-4
Non-hazardous waste disposed [kg] 8.09E+2 1.00E+1 1.63E+2
Radioactive waste disposed [kg] 9.50E-2 9.68E-5 4.89E-4
Components for re-use [kg] 0.00E+0 0.00E+0 0.00E+0
Materials for recycling [kg] 0.00E+0 9.90E+2 0.00E+0
Materials for energy recovery [kg] 0.00E+0 0.00E+0 0.00E+0
Exported electrical energy [MJ] 0.00E+0 0.00E+0 0.00E+0
Exported thermal energy [MJ] 0.00E+0 0.00E+0 0.00E+0
Interpretation
The production stage is the highest contributing stage in the life cycle of Hot Dip Galvanized. Module C3 has a
low contribution while module D presents negative contribution (credit) for all impact categories except ODP.
Due to the Hot-Rolled Steel Coil input, the Pickling is the most contributing stage in all environmental categories
except ADPE, in which Galvanization is the process with the highest contribution due to the zinc coating.
Module D has a significant part for the results, especially for GWP and ADPE (expressive only in Hot-Rolled Steel
Coil). This is because the external scrap input is low, which increase the net scrap value, reducing the original
impact of the production (A1-A3).
Total use of renewable primary energy carrier (PERT) and total use of non-renewable primary energy (PENRT)
are dominated by the extraction and processing of raw materials and the generation of electricity, steam and heat
from primary energy resources, including extraction, refining and transport.
In general, the main contribution to primary energy in the blast furnace/basic oxygen furnace (BF/BOF) route
comes from the use of coal/coke as an energy and carbon source.
References
PCR part A Assessment and Requirements on the Background
Product Category Rules for Construction Products. Report. Berlin: Institut Bauen und Umwelt e.V. (IBU),
Part A: Calculation Rules for the Life Cycle 2013.
NBR 7008-2
PCR part B ABNT NBR 7008-2:2012, Steel-coated coils and plates
Product Category Rules for Construction Products. with zinc or zinc-iron alloy by hot-dip continuous
Part B: Requirements on the EPD for Structural Steel. process immersion Part 2: Commercial quality steel
Berlin: Institut Bauen und Umwelt e.V. (IBU), 2014. stamping
ArcelorMittal Vega, 2019. Available online: NBR 7008-3
https://brasil.arcelormittal.com/a-arcelormittal/quem- ABNT NBR 7008-3:2012, Steel-coated coils and plates
somos/arcelormittal-vega with zinc or zinc-iron alloy by hot-dip continuous
process immersion Part 3: Structural steels
European Commission Technical Steel Research,
Sansom, M. and Meijer, J.: Life-cycle assessment
(LCA) for steel construction, 2001-12 ISO 14040
DIN EN ISO 14040:2009-11, Environmental
GaBI ts Software management - Life cycle assessment - Principles and
GaBi 8.7. Software System and Holistic Accounting framework
Database, Version 8.7.0.18. Stuttgart, Echterdingen:
thinkstep AG, Service Package/SP 37 [accessed ISO 14044
01.10.2019]. DIN EN ISO 14044:2006-10, Environmental
management - Life cycle assessment - Requirements
GaBI ts Documentation and guidelines
Documentation of the GaBi datasets for Life Cycle
Engineering. LBP, Universitity of Stuttgart and PE EN 15804
International, 2017. http://documentation.gabi- EN 15804:2012-04+A1 2013/, Sustainability of
software.com. construction works — Environmental Product
Declarations — Core rules for the product category of
Worldsteel 2014 construction products
Worldsteel 2014: A methodology to determine the LCI
of steel industry co-products.
https://www.worldsteel.org/en/dam/jcr:167ec6bc-d974-
4405-8d53-56825ad4552f/Co-
product+methodology+for+the+steel+industry+2014.pd
f
6 Environmental Product Declaration ArcelorMittal Brasil – Hot Dip Galvanized
Publisher
Institut Bauen und Umwelt e.V. Tel +49 (0)30 3087748- 0
Panoramastr. 1 Fax +49 (0)30 3087748- 29
10178 Berlin Mail info@ibu-epd.com
Germany Web www.ibu-epd.com
Programme holder
Institut Bauen und Umwelt e.V. Tel +49 (0)30 - 3087748- 0
Panoramastr 1 Fax +49 (0)30 – 3087748 - 29
10178 Berlin Mail info@ibu-epd.com
Germany Web www.ibu-epd.com
Author of the Life Cycle
Assessment Tel +55 (11) 2349-3006
Espaço Eco Foundation Fax 0
Estrada Ribeirão do Soldado 230 Mail espacoeco@basf.com
982201 São Bernardo do Campo, Web www.espacoeco.org.br/
SP – Brasil
Brazil
Owner of the Declaration
ArcelorMittal Brasil Tel 0800 015 1221
Av. Carandaí, 1115 - Funcionários Fax -
25 an Mail
30130 -915 - Belo Horizonte arcelormittalnet@arcelormittal.co
Brazil m.br
Web
http://www.arcelormittal.com.b
r/
