ENVIRONMENTAL PRODUCT DECLARATION
as per ISO 14025 and EN 15804+A2
Owner of the Declaration Kingspan Insulation B.V.
Publisher Institut Bauen und Umwelt e.V. (IBU)
Programme holder Institut Bauen und Umwelt e.V. (IBU)
Declaration number EPD-KIN-20230169-CBA1-EN
Issue date 11/07/2023
Valid to 10/07/2028
Therma™ TW58
Kingspan Insulation B.V.
www.ibu-epd.com | https://epd-online.com
General Information
Kingspan Insulation B.V. Therma™ TW58
Programme holder Owner of the declaration
IBU – Institut Bauen und Umwelt e.V. Kingspan Insulation B.V.
Hegelplatz 1 Lingewei 8
10117 Berlin 4004LL Tiel
Germany Netherlands
Declaration number Declared product / declared unit
EPD-KIN-20230169-CBA1-EN Therma™ TW58
1m2, 120mm thickness, R = 5,45 m2.K/W
D
This declaration is based on the product category rules: Scope:
Insulating materials made of foam plastics, 01/08/2021 The insulation material Therma™ TW58 is produced by Kingspan
(PCR checked and approved by the SVR) Insulation at the manufacturing facility in Kankaanpää (Finland).
Therma™ TW58 is an insulation board with a rigid thermoset
Issue date polyisocyanurate (PIR) fibre-free insulation core, faced on both sides with
a low emissivity composite foil. Therma™ TW58 Concrete element
11/07/2023
insulation is used as thermal insulation in the industrial production of
concrete elements.
Valid to
In order to enable the user of the EPD to calculate the LCA results for
10/07/2028 different thicknesses, the EPD contains the respective calculation rules.
The owner of the declaration shall be liable for the underlying information
and evidence; the IBU shall not be liable with respect to manufacturer
information, life cycle assessment data and evidences.
The EPD was created according to the specifications of EN 15804+A2. In
the following, the standard will be simplified as EN 15804.
Verification
The standard EN 15804 serves as the core PCR
Independent verification of the declaration and data according to ISO
14025:2011
Dipl.-Ing. Hans Peters
(Chairman of Institut Bauen und Umwelt e.V.) internally X externally
Florian Pronold Vito D'Incognito,
(Managing Director Institut Bauen und Umwelt e.V.) (Independent verifier)
1 Environmental Product Declaration - Kingspan Insulation B.V. - Therma™ TW58
Product
characteristics according to EN 13165 - Thermal insulation
Product description/Product definition products for buildings - Factory made rigid polyurethane foam
Therma™ TW58 is an insulation board with a rigid thermoset (PU) products - Specification
polyisocyanurate (PIR) fibre-free insulation core, faced on both The declaration of performance of the product can be found at
sides with a low emissivity composite foil. The product is www.kingspan.com.
available in variable thicknesses from 20 mm up to 200 mm.
This EPD is based on a thickness of 120 mm and R -value of Base materials/Ancillary materials
D
5,45 m²·K/W. For the placing on the market of the product in the The product contains approximately 3,3 kg/m2 polyurethane
European Union/European Free Trade Association (EU/EFTA) rigid foam and 0,3 kg/m2 multi-layer aluminium facings. The
(with the exception of Switzerland) Regulation (EU) No. main materials of the polyurethane foam are MDI (between 57-
305/2011 (CPR) applies. The product needs a declaration of 62 %), polyol (between 27-32 %) and a blowing agent (between
performance taking into consideration EN 13165 - Thermal 5-6 %). Due to the closed cell structure (conform EN 13165),
insulation products for buildings - Factory made polyurethane the blowing agent remains in the foam. Water, flame retardants
foam (PU) products - specification and the CE-marking. For the and additives are added (between 4-8 %).
application and use the respective national provisions apply. In the current REACH regulations, polyurethane foam insulation
products are considered 'articles' and are exempt from the
Application requirements of Articles 57 and 59(1) of REACH Regulation
Therma™ TW58 Concrete element insulation is used as (EC) No 1907/2006. These products are not classified as
thermal insulation in the industrial production of concrete 'hazardous products' according to any current legislation, and
elements. can hence be declared as follows:
- This article contains substances listed in the candidate list
Technical Data
(date: 31.08.2022) exceeding 0.1 percentage by mass: no.
Constructional data - This article contains other carcinogenic, mutagenic, reprotoxic
(CMR) substances in categories 1A or 1B which are not on the
Name Value Unit
candidate list, exceeding 0.1 percentage by mass: no.
Thermal conductivity according to EN
0.022 W(m.K) - Biocide products were added to this construction product or it
13165
has been treated with biocide products (this then concerns a
Reaction to fire acc. to EN 13165 F treated product as defined by the (EU) Biocidal Products
CS(10\Y) Regulation No. 528/2012 (BPR): no.
Compressive strength acc. to EN 13165
100
Reference service life
Thickness tolerance according to EN
13165 T2 The reference service life is not to be declared in this EPD as it
does not cover the use stage.
Performance data of the product in accordance with the
declaration of performance with respect to its essential
LCA: Calculation rules
covers:
Declared Unit · A1, raw material extraction and processing, processing of
The declared unit (1 m²) and conversion factors are listed in the secondary material input (e.g. recycling processes),
table below. · A2, transport to the manufacturer,
Declared unit · A3, manufacturing, including provision of all materials,
products and energy, packaging processing and its transport,
Name Value Unit
as well as waste processing up to the end-of-waste state or
Declared unit 1 m2 disposal of final residues during the product stage.
Gross density 30 kg/m3
Grammage 3.6 kg/m2 The construction process stage includes:
· A4 transport to the building site;
Layer thickness 0.12 m
· A5 installation in the building including provision of all
The scope of this EPD is the thermal insulation product materials, products and energy, as well as waste processing up
Therma™ TW58 as produced by Kingspan Insulation at the to the end-of-waste state or disposal of final residues during the
manufacturing facility in Kankaanpää (Finland). The construction process stage.
environmental impacts have been calculated over the calendar
year 2021. The end-of-life stage is a mandatory information module and it
covers:
The EPD is studied for a common product thickness of 120 · C1 de-construction, demolition;
mm. Multiplication factors are included to calculate impacts for · C2 transport to waste processing;
other product thicknesses within the range of 20 to 200 mm. · C3 waste processing for reuse, recovery and/or recycling;
· C4 disposal (not applicable for this EPD) including provision
and all transport, provision of all materials, products and related
System boundary
energy and water use.
The type of EPD according to EN 15804 is:
cradle to gate with options, modules C1–C4, and module D Environmental burden of the incineration (R1 > 60 %) of the
(A1–A3, C, D and additional modules: A4, A5). product at the end-of-life stage are assigned to the product
system (C3); resulting potential credits for thermal and electrical
The product stage is a mandatory information module and it energy from energy substitution are declared in module D.
2 Environmental Product Declaration - Kingspan Insulation B.V. - Therma™ TW58
into account.
Geographic Representativeness
Land or region, in which the declared product system is Background database
manufactured, used or handled at the end of the product´s Background data from GaBi ts Version 10 is used with GaBi
lifespan: Europe data sets CUP2022.1.
Period under review
Comparability
The input data for raw material production and the consumption
Basically, a comparison or an evaluation of EPD data is only
of process energy on the manufacturing facility was measure
possible if all the data sets to be compared were created
data during January 1st 2021 to December 31st 2021, i.e.
according to EN 15804 and the building context, respectively
collected over a 12 month period.
the product-specific characteristics of performance, are taken
LCA: Scenarios and additional technical information
Installation into the building (A5)
Characteristic product properties of biogenic carbon
The total mass of biogenic carbon containing materials is less Name ValueUnit
than 5 % of the total mass of the product and accompanying Output substances following waste treatment on
0.106 kg
packaging. site
The recycling of the packaging is considered in A5.
Technical information
The following technical information is a basis for the declared End of life (C1-C4)
modules or can be used for developing specific scenarios in the The assumptions for C1 are: diesel driven excavator (100 kW;
context of a building assessment. 0.2 litre fuel per ton excavated material). The assumptions for
C2 are: Truck Euro 6, diesel driven, 26-28 t gross weight,
Manufacturing (A3) assumed distance 50 km
A polyethylene packaging foil is used. The products are Name ValueUnit
transported on wooden pallets.
Collected as mixed construction waste 3.6 kg
Within Module A3 the following packaging of the final product is
Energy recovery 3.975 kg
included:
Recycling (aluminium content of the multi-layer
- Polyethylene cover and wrap: 0,038 kg/m² - Wooden pallet: 0.025 kg
aluminium facings)
0,068 kg/m²
Transport to the building site (A4) Reuse, recovery and/or recycling potentials (D), relevant
scenario information
Name Value Unit
Waste incineration with energy recuperation is assumed as
Litres of fuel 0.0103 l/100km
end-of-life scenario
Transport distance 100 km
Gross density of products transported 30 kg/m3
3 Environmental Product Declaration - Kingspan Insulation B.V. - Therma™ TW58
LCA: Results
DESCRIPTION OF THE SYSTEM BOUNDARY (X = INCLUDED IN LCA; ND = MODULE OR INDICATOR NOT DECLARED; MNR =
MODULE NOT RELEVANT)
Benefits and
Construction loads beyond
Product stage Use stage End-of-life stage
process stage the system
boundaries
la ire ta m w a Ry lp p u s tro p s n a rT g n iru tc a fu n a M e h t m o rf tro p s n a rTe tis e h t o t e ta g y lb m e s s A e s U e c n a n e tn ia M ria p e R tn e m e c a lp e R tn e m h s ib ru fe R y g re n e la n o ita re p Oe s u re ta w la n o ita re p Oe s u n o itc u rts n o c -e Dn o itilo m e d tro p s n a rT g n is s e c o rp e ts a W la s o p s iD -e s u e R-y re v o c e R-g n ilc y c e Rla itn e to p
A1 A2 A3 A4 A5 B1 B2 B3 B4 B5 B6 B7 C1 C2 C3 C4 D
X X X X X MND MND MNR MNR MNR MND MND X X X X X
RESULTS OF THE LCA - ENVIRONMENTAL IMPACT according to EN 15804+A2: 1m2 120mm Therma™ TW58
Parameter Unit A1-A3 A4 A5 C1 C2 C3 C4 D
GWP-total kg CO 2 eq 1.05E+01 3.03E-02 2.19E-01 2.31E-03 1.52E-02 7.79E+00 0 -3.2E+00
GWP-fossil kg CO 2 eq 1.08E+01 3.02E-02 9.67E-02 2.31E-03 1.51E-02 7.63E+00 0 -3.19E+00
GWP-biogenic kg CO 2 eq -3.27E-01 -4.17E-05 1.22E-01 3.09E-06 -2.08E-05 1.66E-01 0 -1.58E-02
GWP-luluc kg CO 2 eq 7.92E-03 1.68E-04 1.36E-06 2.85E-08 8.41E-05 1.43E-05 0 -3.64E-04
ODP kg CFC11 eq 1.21E-11 1.81E-15 2.61E-14 1.41E-16 9.04E-16 5.77E-13 0 -2.05E-11
AP mol H+ eq 2.28E-02 3.11E-05 2.92E-05 1.07E-05 1.56E-05 4.55E-03 0 -4.9E-03
EP-freshwater kg P eq 4.42E-05 9.01E-08 6.47E-09 4.65E-10 4.5E-08 1.56E-07 0 -4.21E-06
EP-marine kg N eq 5.9E-03 1.02E-05 8.87E-06 5.1E-06 5.09E-06 2.2E-03 0 -1.18E-03
EP-terrestrial mol N eq 6.14E-02 1.21E-04 1.37E-04 5.59E-05 6.05E-05 2.53E-02 0 -1.27E-02
kg NMVOC
POCP 2.67E-02 2.74E-05 2.46E-05 1.45E-05 1.37E-05 5.64E-03 0 -3.35E-03
eq
ADPE kg Sb eq 1.02E-05 2.52E-09 6.38E-10 9.44E-11 1.26E-09 1.58E-08 0 -4.66E-07
ADPF MJ 2.77E+02 4.03E-01 6.05E-02 3.12E-02 2.02E-01 2.02E+00 0 -5.33E+01
m3 world eq
WDP 1.55E+00 2.71E-04 2.18E-02 4.29E-06 1.35E-04 7.72E-01 0 -3.5E-01
deprived
GWP = Global warming potential; ODP = Depletion potential of the stratospheric ozone layer; AP = Acidification potential of land and water; EP =
Eutrophication potential; POCP = Formation potential of tropospheric ozone photochemical oxidants; ADPE = Abiotic depletion potential for non-fossil
resources; ADPF = Abiotic depletion potential for fossil resources; WDP = Water (user) deprivation potential)
RESULTS OF THE LCA - INDICATORS TO DESCRIBE RESOURCE USE according to EN 15804+A2: 1m2 120mm Therma™
TW58
Parameter Unit A1-A3 A4 A5 C1 C2 C3 C4 D
PERE MJ 2.49E+01 2.29E-02 1.04E+00 1.18E-04 1.15E-02 3.54E-01 0 -1.52E+01
PERM MJ 1.02E+00 0 -1.02E+00 0 0 0 0 0
PERT MJ 2.59E+01 2.29E-02 1.49E-02 1.18E-04 1.15E-02 3.54E-01 0 -1.52E+01
PENRE MJ 1.65E+02 4.04E-01 1.7E+00 3.13E-02 2.02E-01 1.13E+02 0 -5.34E+01
PENRM MJ 1.12E+02 0 -1.63E+00 0 0 -1.11E+02 0 0
PENRT MJ 2.77E+02 4.04E-01 6.06E-02 3.13E-02 2.02E-01 2.02E+00 0 -5.34E+01
SM kg 0 0 0 0 0 0 0 0
RSF MJ 0 0 0 0 0 0 0 0
NRSF MJ 0 0 0 0 0 0 0 0
FW m3 7.59E-02 2.59E-05 5.14E-04 1.78E-07 1.3E-05 1.82E-02 0 -1.64E-02
PERE = Use of renewable primary energy excluding renewable primary energy resources used as raw materials; PERM = Use of renewable primary
energy resources used as raw materials; PERT = Total use of renewable primary energy resources; PENRE = Use of non-renewable primary energy
excluding non-renewable primary energy resources used as raw materials; PENRM = Use of non-renewable primary energy resources used as raw
materials; PENRT = Total use of non-renewable primary energy resources; SM = Use of secondary material; RSF = Use of renewable secondary fuels;
NRSF = Use of non-renewable secondary fuels; FW = Use of net fresh water
RESULTS OF THE LCA – WASTE CATEGORIES AND OUTPUT FLOWS according to EN 15804+A2:
1m2 120mm Therma™ TW58
Parameter Unit A1-A3 A4 A5 C1 C2 C3 C4 D
HWD kg 1.11E-07 1.94E-12 5.38E-12 1.03E-13 9.68E-13 2.76E-10 0 -6.6E-09
NHWD kg 2.88E-01 5.79E-05 9.41E-03 2.93E-06 2.9E-05 4.37E-02 0 -8.04E-02
RWD kg 4.93E-03 4.98E-07 2.97E-06 3.43E-08 2.49E-07 8.4E-05 0 -4.17E-03
CRU kg 0 0 0 0 0 0 0 0
MFR kg 0 0 0 0 0 2.54E-02 0 0
MER kg 0 0 1.06E-01 0 0 3.46E+00 0 0
EEE MJ 0 0 3.5E-01 0 0 1.32E+01 0 0
EET MJ 0 0 6.28E-01 0 0 2.36E+01 0 0
4 Environmental Product Declaration - Kingspan Insulation B.V. - Therma™ TW58
HWD = Hazardous waste disposed; NHWD = Non-hazardous waste disposed; RWD = Radioactive waste disposed; CRU = Components for re-use;
MFR = Materials for recycling; MER = Materials for energy recovery; EEE = Exported electrical energy; EET = Exported thermal energy
RESULTS OF THE LCA – additional impact categories according to EN 15804+A2-optional:
1m2 120mm Therma™ TW58
Parameter Unit A1-A3 A4 A5 C1 C2 C3 C4 D
Disease
PM 2.06E-07 1.8E-10 2.3E-10 1.21E-10 8.98E-11 1.27E-08 0 -4.26E-08
incidence
IR kBq U235 eq 5.54E-01 7.3E-05 4.47E-04 4.99E-06 3.65E-05 1.35E-02 0 -7.13E-01
ETP-fw CTUe 1.13E+02 2.8E-01 3.63E-02 2.17E-02 1.4E-01 6.96E-01 0 -1.21E+01
HTP-c CTUh 7.24E-09 5.64E-12 2.17E-12 4.02E-13 2.82E-12 5.21E-11 0 -6.28E-10
HTP-nc CTUh 6.28E-07 2.93E-10 1.69E-10 2.03E-11 1.46E-10 1.9E-09 0 -2.21E-08
SQP SQP 8.31E+01 1.39E-01 1.65E-02 8.61E-05 6.94E-02 4.26E-01 0 -9.2E+00
PM = Potential incidence of disease due to PM emissions; IR = Potential Human exposure efficiency relative to U235; ETP-fw = Potential comparative
Toxic Unit for ecosystems; HTP-c = Potential comparative Toxic Unit for humans (cancerogenic); HTP-nc = Potential comparative Toxic Unit for humans
(not cancerogenic); SQP = Potential soil quality index
Disclaimer 1 – for the indicator 'Potential Human exposure efficiency relative to U235'.This impact category deals mainly with the
eventual impact of low-dose ionizing radiation on human health of the nuclear fuel cycle. It does not consider effects due to possible
nuclear accidents, occupational exposure or to radioactive waste disposal in underground facilities. Potential ionizing radiation from the
soil, radon and from some construction materials is also not measured by this indicator.
Disclaimer 2 – for the indicators 'abiotic depletion potential for non-fossil resources', 'abiotic depletion potential for fossil resources',
'water (user) deprivation potential, deprivation-weighted water consumption', 'potential comparative toxic unit for ecosystems', 'potential
comparative toxic unit for humans – cancerogenic', 'Potential comparative toxic unit for humans - not cancerogenic', 'potential soil
quality index'. The results of this environmental impact indicator shall be used with care as the uncertainties on these results are high
as there is limited experience with the indicator.
Factors for different thicknesses
The LCA results for the insulation material declared in this EPD refer to a product with a thickness of 120 mm. To enable the user of the
EPD to calculate the results for different thicknesses the factors in the following table can be used for the calculation. The LCA results
in chapter 5 have to be multiplied with these factors.
This EPD was created using a software tool.
References
Biocidal Products Regulation No. 528/2012 (BPR) Specification
Regulation (EU) No 528/2012 of the European Parliament and
of the Council of 22 May 2012 concerning the making available EN 15804
on the market and use of biocidal products EN 15804:2012+A2:2019+AC:2021, Sustainability of
construction works — Environmental Product Declarations —
CPR Core rules for the product category of construction products.
Regulation (EU) No. 305/2011 of the European Parliament and
of the Council of 9 March 2011 laying down harmonised GaBi ts
condition for the marketing of construction products and thinkstep AG: Leinfelden-Echterdingen GaBi Software- System
repealing Council Directive 89/106/EC and Database for Life Cycle Engineering 1992- 2019
ISO 14025 IBU 2022
EN ISO 14025:2011, Environmental labels and declarations — Institut Bauen und Umwelt e.V.: General Instructions for the
Type III environmental declarations — Principles and EPD programme of Institut Bauen und Umwelt e.V., Version
procedures. 2.1, Berlin: Institut Bauen und Umwelt e.V., 2022. www.ibu-
epd.com
EN 13165
EN 13165:2012+A2:2016: Thermal insulation products for LCA-tool
buildings. Factory made polyurethane foam (PU) products. Kingspan LCA tool, version 1.1. IBU-KSI-202001-LT1- EN.
5 Environmental Product Declaration - Kingspan Insulation B.V. - Therma™ TW58
Developed by Sphera Solutions GmbH (formely Thinkstep Environmental Product Declarations of Institut Bauen und
GmbH) Umwelt (IBU), Part B: Requirements on the EPD for insulating
materials made of foam plastics. May 2023
PCR Version 1.7, Part A
Institut Bauen und Umwelt e.V., Berlin (pub.): Product Category REACH
Rules for Building-Related Products and services, Part A: Regulation (EC) No 1907/2006 of the European Parliament and
Calculation Rules for the Life Cycle Assessment and of the Council on the Registration, Evaluation, Authorisation
Requirements on the Project Report according to EN and Restriction of Chemicals (REACH)
15804+A2:2019 November 2021 https://echa.europa.eu/candidate-list-table;
PCR 2023, Part B Candidate list
Institut Bauen und Umwelt e.V., Berlin (pub.): Product Category https://echa.europa.eu/candidate-list-table; accessed
Rules for Construction Products from the range of 31.08.2022, 233 substances listed.
6 Environmental Product Declaration - Kingspan Insulation B.V. - Therma™ TW58
Publisher
Institut Bauen und Umwelt e.V. +49 (0)30 3087748- 0
Hegelplatz 1 info@ibu-epd.com
10117 Berlin www.ibu-epd.com
Germany
Programme holder
Institut Bauen und Umwelt e.V. +49 (0)30 3087748- 0
Hegelplatz 1 info@ibu-epd.com
10117 Berlin www.ibu-epd.com
Germany
Author of the Life Cycle Assessment
Kingspan Insulation B.V. +31 (0) 543 543 210
Lingewei 8 info@kingspaninsulation.nl
4004LL Tiel www.kingspan.com
Netherlands
Owner of the Declaration
Kingspan Insulation B.V. +31 (0) 543 543 210
Lingewei 8 info@kingspaninsulation.nl
4004LL Tiel www.kingspan.com
Netherlands
7 Environmental Product Declaration - Kingspan Insulation B.V. - Therma™ TW58
