ENVIRONMENTAL PRODUCT DECLARATION
as per ISO 14025 and EN 15804+A2
Owner of the Declaration Knauf Ceiling Solutions GmbH & Co. KG
Publisher Institut Bauen und Umwelt e.V. (IBU)
Programme holder Institut Bauen und Umwelt e.V. (IBU)
Declaration number EPD-KNA-20220025-IBD2-EN
Issue date 30.03.2022
Valid to 29.03.2027
Metal Ceiling Membranes (0.6 mm, with acoustic fleece)
Knauf Ceiling Solutions GmbH & Co. KG
www.ibu-epd.com | https://epd-online.com
1. General Information
Knauf Ceiling Solutions GmbH & Co. KG Metal Ceiling Membranes (0.6 mm, with acoustic
fleece)
Programme holder Owner of the declaration
IBU – Institut Bauen und Umwelt e.V. Knauf Ceiling Solutions GmbH & Co. KG
Hegelplatz 1 Elsenthal 15
10117 Berlin 94481 Grafenau
Germany Germany
Declaration number Declared product / declared unit
EPD­KNA­20220025­IBD2­EN 1 m² average steel ceiling membrane with a thickness of 0.6 mm and a
surface weight of 4.73 kg/m² (with acoustic fleece)
This declaration is based on the product category rules: Scope:
Metal ceilings, 01.08.2021 This document refers to average steel ceiling membranes with a thickness
(PCR checked and approved by the SVR) of 0.6 mm and a surface weight of 4.73 kg/m² (with acoustic fleece).
The products are manufactured at the following production sites of Knauf
Issue date Ceiling Solutions GmbH & Co. KG:
­ Rankweil (Austria)
30.03.2022
­ Stafford (United Kingdom)
The owner of the declaration shall be liable for the underlying information
Valid to
and evidence; the IBU shall not be liable with respect to manufacturer
29.03.2027 information, life cycle assessment data and evidences.
The EPD was created according to the specifications of EN 15804+A2. In
the following, the standard will be simplified as EN 15804.
Verification
The standard EN 15804 serves as the core PCR
Independent verification of the declaration and data according to ISO
14025:2011
internally X externally
Dipl.­Ing. Hans Peters
(Chairman of Institut Bauen und Umwelt e.V.)
Florian Pronold Matthias Schulz,
(Managing Director Institut Bauen und Umwelt e.V.) (Independent verifier)
1 Environmental Product Declaration ­ Knauf Ceiling Solutions GmbH & Co. KG ­ Metal Ceiling Membranes (0.6 mm, with acoustic fleece)
2. Product
2) 'This product contains other carcinogenic, mutagenic,
2.1 Product description/Product definition reprotoxic (CMR) substances in categories 1A or 1B which are
Knauf Ceiling Solutions metal ceiling systems are made from not on the candidate list, exceeding 0.1 percentage by mass':
punched and formed galvanised steel, as comprehensive No.
construction kits or individual components and industrially
manufactured. The construction kit comprises the visible 3) 'Biocide products were added to this construction product or
membrane and the substructure. The membranes (tiles, panels, it has been treated with biocide products (this then concerns a
bulkheads) are offered with various edge details and delivered treated product as defined by the (EU) Ordinance on Biocide
unperforated or with a range of perforation patterns, fulfilling the Products No. 528/2012': No.
functional requirements. The substructure is either exposed or
concealed. 2.6 Manufacture
The system components for metal ceilings are manufactured in
For the placing on the market of the product in the European a continuous manufacturing process. The sheet steel comes
Union/European Free Trade Association (EU/EFTA) (with the mainly in coils, gets optionally perforated, afterwards cut to
exception of Switzerland) Regulation (EU) No. 305/2011 (CPR) size, punched, formed and powder­coated after the cleaning
applies. The product needs a declaration of performance taking process. Punching and perforation waste is gathered, collected
into consideration EN 13964:2014, suspended ceiling by local disposal companies, and redirected to the recycling
requirements and test methods and the CE­marking and centres. The acoustic fleece gets applied to the back in a
UKCA­marking (in the UK). continuous process. All production steps are carried out in
For the application and use the respective national provisions accordance with the requirements and test guidelines outlined
apply. in EN 13964.
2.2 Application The manufacturing plants are certified according to ISO 9001
The described metal solutions are typically used internally as and ISO 14001.
design elements, to cover the ceiling void, as well as acoustic
solutions for sound absorption and sound attenuation, for fire 2.7 Environment and health during manufacturing
resistance and against fire spreading, for cleanrooms and high Manufacturing conditions do not demand any particular health
hygiene requirements. protection measures with the exception of those designated by
the authorities for special working areas, e.g., high­visibility
2.3 Technical Data vests, ear protection, safety shoes.
Metal membranes are regulated by EN 13964 and have The threshold limit values are not exceeded at any point in the
corresponding labelling and declaration of performance. production process. Waste emissions generated during
The following data provide an overview of results: production are cleaned in accordance with statutory
Constructional data requirements. Emissions are below those outlined in the
Technical Guidelines governing Air. Water/ground: No
Name Value Unit
contamination of water or soil occurs. All the values established
Sound absorption coefficient (ISO 354, ISO ≤
% inside and outside the production facilities are below the
11654) 0.75(L)
applicable requirements governing noise protection in the UK
Airborne sound reduction (EN 20140­9, ISO and Austria. Noise­intensive plant components such as
≤ 21 dB
140­3) perforation lines are isolated accordingly by structural
Grammage 4.73 kg/m2 measures. ISO 14001 certificates and other manufacturer­
specific documents on environment protection can be
Release of formaldehyde (EN 13964) E1 ­
requested from the manufacturer.
Durability class (EN 13964) B ­
Further characteristics according to the PCR are not relevant 2.8 Product processing/Installation
for this product. There are no recognised systemic hazards associated with the
installation of ceiling membranes. Metal ceiling membranes are
The performance data of the product, with respect to its suspended by a substructure.
essential characteristics, is in accordance with the declaration Installation must be carried out by trained personnel. Workers
of performance according to EN 13964:2014, suspended should wear appropriate personal protective equipment.
ceiling requirements and test methods. Equipment such as gloves and goggles are recommended to
prevent skin irritation.
2.4 Delivery status
The metal ceiling systems, construction kits and components 2.9 Packaging
are produced in individual module sizes and can be supplied The membranes are packaged in cardboard boxes with a
with or without substructures. separation paper protecting the visible surface or sealed with
Packaging is usually on pallets and/or in cardboard. transparent polyethylene film. These packages lie on
chemically untreated wooden pallets and are easily separable.
2.5 Base materials/Ancillary materials The pallets are wrapped with polyethylene stretch film. Film,
Name Value Unit paper and wood can be recycled in the usual ways.
Galvanised steel > 96 %
2.10 Condition of use
Surface coating < 3 %
Long service life is based on regular maintenance, care and
Acoustic fleece (cellulose/glass) < 1 % repair of the product. When handled properly, the mechanical
1) 'This product contains substances listed in the candidate list and structural physical properties of the metal membrane
(08.07.2021) exceeding 0.1 percentage by mass': No. remain intact throughout its entire service life. Generally, the
material composition of the product does not alter during the
2 Environmental Product Declaration ­ Knauf Ceiling Solutions GmbH & Co. KG ­ Metal Ceiling Membranes (0.6 mm, with acoustic fleece)
period of use.
Water
2.11 Environment and health during use No environmental influences are known in the case of
There are no known interactions between the product, the unforeseen water ingress. The resistance of the ceiling system
environment and health. Volatile organic compounds are below following the impact of water is dependent on the corrosion
the valuation limit. protection class in which the ceiling system is classified.
2.12 Reference service life
Mechanical destruction
The service life of the metal membranes is for more than 50 In the case of mechanical destruction, all substances remain
years, depending on the area of use, exposure and state of bound. It can be assumed that in the case of coated ceilings,
maintenance. Within the framework of the conditions of use, no possible paint splinters arise in such small volumes that no
ageing effects are to be expected apart from visual negative effects are incurred by the environment.
discolouration caused by air circulation.
2.14 Re-use phase
2.13 Extraordinary effects
The metal ceiling systems can be removed and re­used without
Fire damaging the product. Metal membrane components and
The declared products are classified in the fire reaction class substructure components made of steel can be redirected to
A2­s2, d0 according to EN 13501-1. This means that they are material recycling.
"non­combustible" according to the German building authority
designation (and also many other European countries) with 2.15 Disposal
negligible smoke development and no burning droplets in the In accordance with the Waste Index Act (AVV) and the
event of a fire. European Waste Catalogue (EWC), the waste key for steel as a
Fire reaction component of metal ceiling systems made of steel is: 17­04­05
– Iron and steel.
Name Value
Building material class A2
The waste key for fleece is: 17­04­07 – Construction and
Burning droplets s2 demolition waste.
Smoke gas development d0
2.16 Further information
Further information at www.knaufceilingsolutions.com
3. LCA: Calculation rules
weight of the ceiling membranes directly depends on the
3.1 Declared Unit perforation type. Thus, the recalculation for specific perforations
This EPD refers to a declared unit of 1 m² of average steel based on the product mass is possible.
ceiling membrane with a thickness of 0.6 mm (Standard white
RAL 9010) and a surface weight of 4.73 kg/m² with acoustic 3.2 System boundary
fleece. The life cycle assessment of average metal ceiling membranes
includes a cradle­to­gate analysis of the products'
Declared unit
environmental impacts with modules C1–C4 and module D
Name Value Unit
(A1–A3, + C + D). Subsequent life cycle phases are part of the
Declared unit 1 m2 analysis:
Grammage 4.73 kg/m2
Module A1-A3 | Production stage
The production of the associated gaskets is declared in a
The production stage includes the upstream burdens of raw
separate annexe to this EPD.
material supply, their transports and the manufacturing plants of
Knauf Ceiling Solutions located in Rankweil (AT) and Stafford
The substructure is not part of this EPD.
(UK). The production of metal ceiling membranes includes
punching, stamping and trimming, powder coating and
The ceiling membranes are produced under different brand
packaging. Main raw material inputs, therefore, refer to steel,
names, at the Knauf Ceiling Solutions production sites in
paint for powder coating and fleece infill. Both production sites
Rankweil (AT) and Stafford (UK). The declared product
are supplied with electricity from the national grid and thermal
represents a weighted average of the two production sites
energy from natural gas.
leading to a high representativity of the results.
The packaging of the products is considered in this stage.
Knauf Ceiling Solutions metal ceiling membranes can be
specifically configurated based on the customer's need
Module C1 | Deconstruction and demolition
resulting in more than 100 standard products. The declared
Disassembly of the product is done either manually or using
unit, therefore, refers to a representative product sold in large
smaller tools. Referring energy demand is
quantities. All products are available in various perforation
designs. Ensuring a consistent representation the standard
considered to be negligible.
perforation of 20 % representing the major production
quantities is declared in this EPD (specific weight without
Module C2 | Transport to disposal
perforation: 5.68 kg/m²). This approach ensures the applicability
The transport to the disposal of the material is estimated
of the EPD for specific products as well as the representativity
declaring a 50 km radius to the disposal. In reality, this scenario
of the results.
may vary depending on the actual location of deconstruction
and referring waste treatment.
As the mass of steel represents the decisive factor in the
product's environmental profile, a linear correlation of product
Module C3 | Waste processing
mass and environmental impact is to be expected. The surface
3 Environmental Product Declaration ­ Knauf Ceiling Solutions GmbH & Co. KG ­ Metal Ceiling Membranes (0.6 mm, with acoustic fleece)
Regarding the steel fraction, the material flow reaching module Merl results in an accurate mapping of product­related material
D for recycling is declared as material for recycling in Module and energy flows. This leads to a high quality of foreground
C3. Environmental impacts resulting from the grinding and data collected. Data collection relies on a consistent process
sorting of steel scrap are not included, as referring energy according to ISO 14044.
demand is considered to be negligible. In addition, a loss rate
of 5 % of the processed material is assumed. 95 % of the The technological, geographical and time­related
material can potentially be recycled. For the acoustic fleece representativeness of the database was kept in mind when
inlay the declared scenario assumes landfilling, therefore no selecting background data. Whenever specific data were
environmental impacts from the waste treatment of the fleece missing, either generic datasets or representative average data
inlay are declared in C3. were used instead. The implemented GaBi background
datasets refer to the latest versions available (not more than
Module C4 | Disposal ten years old) and are carefully chosen.
Module C4 refers to the emissions from the disposal of the
losses from waste processing of lost steel as well as the 3.7 Period under review
disposal of the acoustic fleece inlay. The chosen scenario Foreground data were collected for the production year 2020.
therefore includes the environmental burdens of landfilling of 5 The data are based on the volumes produced on an annual
% of the metal material and 100 % of the acoustic fleece inlay. basis.
3.8 Geographic Representativeness
Module D | Benefits and loads beyond the system
boundary Land or region, in which the declared product system is
Module D declares the recycling of the recovered steel (95 % of manufactured, used or handled at the end of the product´s
the product). It includes the potential for substituting primary lifespan: Europe
steel.
3.9 Allocation
3.3 Estimates and assumptions
For foreground data, the calculation of specific input quantities
Assumptions and approximations are applied in case of a lack
is based on the annual production quantity (square meter), e.g.
of representative data. All assumptions and approximations are
for energy input, packaging, etc.. The steel input on product
documented precisely and represent a best­guess
level was calculated based on the mass of steel in the output.
representation of reality. In case of uncertainty, a conservative
approach is chosen.
Background data for the supply chain of the steel are published
3.4 Cut-off criteria by worldsteel (GaBi-databases). Representing an average of
The LCA model covers all available input and output flows, the global steel industry, worldsteel background datasets
which can be represented based on robust data. Data gaps are ensure a good geographical and technological representation
filled with conservative assumptions from average data (when of steel production. All worldsteel datasets are modelled
available) or with generic data and are documented according to the worldsteel LCA methodology, applying the
accordingly. Only data with a contribution lower than 1 % were system expansion approach for the allocation of co­products
cut off. Thus, no data were neglected, of which a substantial from steel production. As a result, these datasets are not fully
impact is to be expected. All relevant data were collected compliant with the requirements of the EN 15804, which
comprehensively. Cut­off material and energy flows were emphasises the so­called partitioning approach applying a
chosen carefully based on their expected quantitative subdivision of environmental impacts according to their physical
contribution as well as potential environmental impacts. Thus, it relationships. Due to a lack of global data calculated based on
can be assumed that the sum of all neglected input flows does the partitioning approach, the worldsteel datasets refer to the
not account for more than 5 % of the total material, water and closest representation of steel production in this context.
energy flows. Additionally, the deviation of the results of the two allocation
approaches is to be expected under 5 % according to Sphera.
3.5 Background data Scrap input is regarded as burden­free.
This study uses generic background data for the evaluation of
3.10 Comparability
upstream environmental impacts from GaBi databases (GaBi
10; 2021.2). Basically, a comparison or an evaluation of EPD data is only
possible if all the data sets to be compared were created
3.6 Data quality according to EN 15804 and the building context, respectively
Data collection is based on product­specific questionnaires. It the product­specific characteristics of performance, are taken
follows an iterative process clarifying questions via e­mail, into account.
telephone calls or in personal/web meetings. Intensive The GaBi background database was used to calculate the LCA
discussions between Knauf Ceiling Solutions and Daxner & (GaBi 10; 2021.2).
4. LCA: Scenarios and additional technical information
Characteristic product properties of biogenic carbon
Information on describing the biogenic Carbon Content at End of life (C1-C4)
factory gate
Name Value Unit
Name ValueUnit
Collected separately (steel) 4.69 kg
Biogenic carbon content in accompanying kg
0.1 Collected separately (fleece infill) 0.04 kg
packaging C
Recycling (steel) 95 % 4.46 kg
The declared product does not contain biogenic carbon. Landfilling (steel) 5 % 0.23 kg
Landfilling (fleece infill) 100 % 0.04 kg
4 Environmental Product Declaration ­ Knauf Ceiling Solutions GmbH & Co. KG ­ Metal Ceiling Membranes (0.6 mm, with acoustic fleece)
Reuse, recovery and/or recycling potentials (D), relevant Name Value Unit
scenario information Net flow of steel scrap 5.37 kg/m²
5 Environmental Product Declaration ­ Knauf Ceiling Solutions GmbH & Co. KG ­ Metal Ceiling Membranes (0.6 mm, with acoustic fleece)
5. LCA: Results
The following table contains the LCA results for a declared unit of 1 m² average steel ceiling membrane with a thickness of 0.6 mm and
a surface weight of 4.73 kg/m² (with acoustic fleece).
Disclaimer:
EP­freshwater: This indicator has been calculated as 'kg P eq' as required in the characterization model (EUTREND model, Struijs et
al., 2009b, as implemented in ReCiPe; http://eplca.jrc.ec.europa.eu/LCDN/developerEF.xhtml).
DESCRIPTION OF THE SYSTEM BOUNDARY (X = INCLUDED IN LCA; ND = MODULE OR INDICATOR NOT DECLARED; MNR =
MODULE NOT RELEVANT)
Benefits and
Construction loads beyond
Product stage Use stage End of life stage
process stage the system
boundaries
la ire ta m w a Ry lp p u s tro p s n a rT g n iru tc a fu n a M e h t m o rf tro p s n a rTe tis e h t o t e ta g y lb m e s s A e s U e c n a n e tn ia M ria p e R tn e m e c a lp e R tn e m h s ib ru fe R y g re n e la n o ita re p Oe s u re ta w la n o ita re p Oe s u n o itc u rts n o c ­e Dn o itilo m e d tro p s n a rT g n is s e c o rp e ts a W la s o p s iD ­e s u e R­y re v o c e R­g n ilc y c e Rla itn e to p
A1 A2 A3 A4 A5 B1 B2 B3 B4 B5 B6 B7 C1 C2 C3 C4 D
X X X MND MND MND MND MNR MNR MNR MND MND X X X X X
RESULTS OF THE LCA - ENVIRONMENTAL IMPACT according to EN 15804+A2: 1 m² ceiling membrane (0.6 mm; 4.73 kg/m²)
Parameter Unit A1-A3 C1 C2 C3 C4 D
Global Warming Potential total (GWP­total) kg CO 2 eq 1.93E+01 0 1.43E­02 0 1.19E­02 ­9.13E+00
Global Warming Potential fossil fuels (GWP­fossil) kg CO 2 eq 1.95E+01 0 1.42E­02 0 1.21E­02 ­9.12E+00
Global Warming Potential biogenic (GWP­biogenic) kg CO 2 eq ­2.62E­01 0 ­1.68E­05 0 ­1.35E­04 ­5.19E­03
Global Warming Potential luluc (GWP­luluc) kg CO 2 eq 1.01E­02 0 1.16E­04 0 1.32E­05 ­2E­04
Depletion potential of the stratospheric ozone layer (ODP) kg CFC11 eq 2.81E­12 0 2.79E­18 0 2.94E­17 ­2.17E­14
Acidification potential of land and water (AP) mol H+ eq 4.83E­02 0 4.69E­05 0 4.08E­05 ­1.62E­02
Eutrophication potential aquatic freshwater (EP­freshwater) kg P eq 2.84E­05 0 4.2E­08 0 9.74E­09 ­1.98E­06
Eutrophication potential aquatic marine (EP­marine) kg N eq 1.25E­02 0 2.15E­05 0 1.02E­05 ­3.13E­03
Eutrophication potential terrestrial (EP­terrestrial) mol N eq 1.33E­01 0 2.4E­04 0 1.12E­04 ­3.16E­02
Formation potential of tropospheric ozone photochemical oxidants kg NMVOC
4.08E­02 0 4.23E­05 0 3.19E­05 ­1.4E­02
(POCP) eq
Abiotic depletion potential for non fossil resources (ADPE) kg Sb eq 8.15E­05 0 1.25E­09 0 8.48E­10 ­2.26E­05
Abiotic depletion potential for fossil resources (ADPF) MJ 2.27E+02 0 1.88E­01 0 1.75E­01 ­8.92E+01
m3 world eq
Water use (WDP) 8.59E+00 0 1.31E­04 0 ­7.05E­05 ­2.48E+01
deprived
RESULTS OF THE LCA - INDICATORS TO DESCRIBE RESOURCE USE according to EN 15804+A2: 1 m² ceiling membrane (0.6
mm; 4.73 kg/m²)
Parameter Unit A1-A3 C1 C2 C3 C4 D
Renewable primary energy as energy carrier (PERE) MJ 2.33E+01 0 1.08E­02 0 1.31E­02 5.61E+00
Renewable primary energy resources as material utilization
MJ 3.74E+00 0 0 0 0 0
(PERM)
Total use of renewable primary energy resources (PERT) MJ 2.71E+01 0 1.08E­02 0 1.31E­02 5.61E+00
Non renewable primary energy as energy carrier (PENRE) MJ 2.18E+02 0 1.89E­01 0 1.75E­01 ­8.92E+01
Non renewable primary energy as material utilization (PENRM) MJ 8.98E+00 0 0 ­5.8E+00 0 0
Total use of non renewable primary energy resources (PENRT) MJ 2.27E+02 0 1.89E­01 ­5.8E+00 1.75E­01 ­8.92E+01
Use of secondary material (SM) kg 4.92E­01 0 0 0 0 5.37E+00
Use of renewable secondary fuels (RSF) MJ 0 0 0 0 0 0
Use of non renewable secondary fuels (NRSF) MJ 0 0 0 0 0 0
Use of net fresh water (FW) m3 2.21E­01 0 1.24E­05 0 3.71E­06 ­5.8E­01
RESULTS OF THE LCA – WASTE CATEGORIES AND OUTPUT FLOWS according to EN 15804+A2:
1 m² ceiling membrane (0.6 mm; 4.73 kg/m²)
Parameter Unit A1-A3 C1 C2 C3 C4 D
Hazardous waste disposed (HWD) kg 1.79E­07 0 9.96E­12 0 3.04E­11 1.95E­08
Non hazardous waste disposed (NHWD) kg 6.09E­01 0 2.97E­05 0 2.75E­01 1.14E+00
Radioactive waste disposed (RWD) kg 1.7E­03 0 3.43E­07 0 1.99E­06 9.67E­06
Components for re­use (CRU) kg 0 0 0 0 0 0
Materials for recycling (MFR) kg 0 0 0 4.46E+00 0 0
Materials for energy recovery (MER) kg 0 0 0 0 0 0
Exported electrical energy (EEE) MJ 0 0 0 0 0 0
Exported thermal energy (EET) MJ 0 0 0 0 0 0
RESULTS OF THE LCA – additional impact categories according to EN 15804+A2-optional:
1 m² ceiling membrane (0.6 mm; 4.73 kg/m²)
6 Environmental Product Declaration ­ Knauf Ceiling Solutions GmbH & Co. KG ­ Metal Ceiling Membranes (0.6 mm, with acoustic fleece)
Parameter Unit A1-A3 C1 C2 C3 C4 D
Disease
Incidence of disease due to PM emissions (PM) 6.18E­07 0 2.66E­10 0 4.49E­10 ­3.08E­07
incidence
Human exposure efficiency relative to U235 (IR) kBq U235 eq 3.53E­01 0 5.02E­05 0 2.81E­04 1.68E­01
Comparative toxic unit for ecosystems (ETP­fw) CTUe 4.7E+01 0 1.4E­01 0 5.37E­02 ­5.76E+00
Comparative toxic unit for humans (carcinogenic) (HTP­c) CTUh 8.62E­09 0 2.83E­12 0 6.37E­12 ­4.95E­09
Comparative toxic unit for humans (noncarcinogenic) (HTP­nc) CTUh 2.77E­07 0 1.66E­10 0 6.47E­10 ­1.1E­07
Soil quality index (SQP) SQP 4.47E+01 0 6.47E­02 0 1.39E­02 1.34E+00
Disclaimer 1 – for the indicator “Potential Human exposure efficiency relative to U235”. This impact category deals mainly with the
eventual impact of low­dose ionizing radiation on human health of the nuclear fuel cycle. It does not consider effects due to possible
nuclear accidents, occupational exposure or radioactive waste disposal in underground facilities. Potential ionizing radiation from the
soil, radon and from some construction materials is also not measured by this indicator.
Disclaimer 2 – for the indicators “abiotic depletion potential for non­fossil resources”, “abiotic depletion potential for fossil resources”,
“water (user) deprivation potential, deprivation­weighted water consumption”, “potential comparative toxic unit for ecosystems”,
“potential comparative toxic unit for humans – cancerogenic”, “Potential comparative toxic unit for humans ­ not cancerogenic”,
“potential soil quality index”. The results of this environmental impact indicator shall be used with care as the uncertainties on these
results are high as there is limited experience with the indicator.
6. LCA: Interpretation
The following interpretation contains a summary of the LCA weight of 4.73 kg/m² with acoustic fleece.
results referenced to a declared unit of 1 m² of average steel
ceiling membrane with a thickness of 0.6 mm and a surface
The comparison of the products' life cycle phases shows a the steel coils represents the major hot spot in all of the impact
clear dominance of the production phase (modules A1­A3). categories considered.
Module C4 declares impacts from landfilling of steel losses Knauf Ceiling Solutions metal ceiling membranes can be
(assumption: 5 % of steel in the product) and the acoustic specifically configurated based on the customer's need
fleece, making up a minor fraction of the total environmental resulting in more than 100 standard products. The conversion
impact of the products. of the LCA results to other material thicknesses than the
declared reference thickness is proportional to the surface
As a result of material recyclability, the steel fraction removed at weight. As a result, the variability of the environmental impacts
the end of life can substitute primary steel. Module D shows the of single products shows a direct correlation to the product
recycling potential of 95 % of the steel in the product at the end weight.
of its life. This results in credits from the substitution of primary
steel. This implies a slight imprecision for the fleece inlay of products
with improved acoustic performance, as the fleece inlay is not
When it comes to the environmental impacts in the production scalable linearly but surface­related.
phase of the ceiling membranes, the upstream supply chain of The analysis shows that the impact of the fleece inlay itself on
7 Environmental Product Declaration ­ Knauf Ceiling Solutions GmbH & Co. KG ­ Metal Ceiling Membranes (0.6 mm, with acoustic fleece)
the overall result is very small. Thus, the linear scaling based representative perforation of 20 %. It is based on primary data
on the surface weight of the membranes is also considered of the two production sites of Knauf Ceiling Solutions located at
applicable for the acoustic products. Rankweil (AT) and Stafford (UK).
The declared environmental impacts represent a weighted Comparably higher environmental impacts at Rankweil can be
average for specific thicknesses of metal ceiling membranes identified in all of the impact categories except for potential
produced by Knauf Ceiling Solutions considering a ozone depletion and water scarcity.
7. Requisite evidence
The relevant paragraph of the suspended ceiling product containing compound is used during the manufacturing
standard (EN 13964) requires formaldehyde emissions process. Metal ceilings covered by this EPD do not contain any
declaration only for products for which a formaldehyde­ formaldehyde­containing compounds.
8. References
Standards cycle assessment – Requirements and guidelines.
EN 13501-1 Further References
EN 13501­1:2019, Classification of construction products and
building elements according to their reaction to fire, Part 1: AVV
Classification with the results of tests on the reaction to fire of AVV, German List of Wastes Ordinance. Regulation on the
construction products. European Waste List.
EN 13964 Candidate list
EN 13964:2014, Suspended ceilings ­ Requirements and test List of substances of very high concern (SVHC) for
methods. authorisation (ECHA Candidate List), 25.06.2020, published
under Article 59(10) of REACH. Helsinki:
EN 15804 European Chemicals Agency.
EN 15804:2012+A2:2019, Sustainability of construction works ­
Environmental product declarations ­ Core rules for the product European Waste Catalogue
category of construction products. Guidance on classification of waste according to EWC­Stat
categories. Supplement to the Manual for the Implementation of
EN 20140-9 the Regulation (EC) No 2150/2002 on Waste Statistics.
EN ISO 20140­9:1993, Acoustics – Measurement of sound Commission of the European Communities, EUROSTAT.
insulation in buildings.
GaBi
ISO 140-3 GaBi 10, Software­System and Database for Life Cycle
EN ISO 140­3:1995, Acoustics – Measurement of sound Engineering. DB 2021.2. Stuttgart, Echterdingen: Sphera,
insulation in buildings. 1992­2021. Available at:
http://documentation.gabi­software.com
ISO 354
EN ISO 354:2003­12, Acoustics ­ Measurement of sound IBU 2021
absorption in reverberant rooms. Institut Bauen und Umwelt e.V.: Allgemeine Anleitung für das
EPD­­Programm des Institut Bauen und Umwelt e.V. (IBU).
ISO 9001 Version 2.0, Berlin: Institut Bauen und Umwelt e.V., 2021.
EN ISO 9001:2015­11, Quality management systems ­ www.ibu­epd.com
Requirements.
Ordinance on Biocide Products
ISO 11654 Regulation (EU) No 528/2012 of the European Parliament and
EN ISO 11654:1997­07, Acoustics ­ Sound absorbers for use in of the Council of 22 May 2012 concerning the making available
buildings ­ Evaluation of sound absorption. on the market and use of biocidal products.
ISO 14001 PCR part A
EN ISO 14001:2015­11, Environmental management systems ­ Product category rules for building­­related products and
Requirements with guidance for use. services. Part A: Calculation Rules for the Life Cycle
Assessment and Requirements on the Project Report according
ISO 14025 to EN 15804+A2:2019. Version 1.1.
DIN EN ISO 14025:2011­10, Environmental labels and Berlin: Institut Bauen und Umwelt e.V., 2021.
declarations ­ Type III environmental declarations ­ Principles
and procedures. PCR: Metal ceilings
Product category rules for building­related products and
ISO 14044 services. Part B: EPD requirements for metal ceilings. Version
EN ISO 14044:2006­10, Environmental management – Life 1.7. Berlin: Institut Bauen und Umwelt e.V., 08.01.2019.
8 Environmental Product Declaration ­ Knauf Ceiling Solutions GmbH & Co. KG ­ Metal Ceiling Membranes (0.6 mm, with acoustic fleece)
Publisher
Institut Bauen und Umwelt e.V. +49 (0)30 3087748­ 0
Hegelplatz 1 info@ibu­epd.com
10117 Berlin www.ibu­epd.com
Germany
Programme holder
Institut Bauen und Umwelt e.V. +49 (0)30 3087748­ 0
Hegelplatz 1 info@ibu­epd.com
10117 Berlin www.ibu­epd.com
Germany
Author of the Life Cycle Assessment
Daxner & Merl GmbH +43 676 849477826
Lindengasse 39/8 office@daxner­merl.com
1070 Wien www.daxner­merl.com
Austria
Owner of the Declaration
Knauf Ceiling Solutions GmbH & Co. KG 0049 8552 422 0
Elsenthal 15 ceiling.solutions@knauf.com
94481 Grafenau www.knaufceilingsolutions.com
Germany
9 Environmental Product Declaration ­ Knauf Ceiling Solutions GmbH & Co. KG ­ Metal Ceiling Membranes (0.6 mm, with acoustic fleece)
