ENVIRONMENTAL PRODUCT DECLARATION
as per ISO 14025 and EN 15804+A2
Owner of the Declaration Etex
Programme holder Institut Bauen und Umwelt e.V. (IBU)
Publisher Institut Bauen und Umwelt e.V. (IBU)
Declaration number EPD-ETE-20220190-ICA2-EN
Issue date 31.10.2022
Valid to 23.10.2027
Cedral sidings
ETEX
www.ibu-epd.com | https://epd-online.com
Umwelt Produktdeklaration Name des Herstellers – Name des Produkts
1. General Information
Etex Lithuania Cedral sidings
Programme holder Owner of the declaration
IBU – Institut Bauen und Umwelt e.V. Etex Lithuania
Hegelplatz 1 J. Dalinkevičiaus str. 2H
10117 Berlin Naujoji Akmené, 85118
Germany
Declaration number Declared product / declared unit
EPD-ETE-20220190-ICA2-EN Covering 1 m2 of wall with Cedral sidings, over a
reference service life of 60 years.
This declaration is based on the product Scope:
category rules: This EPD presents the Cedral fibre cement sidings.
Fibre cement / Fibre concrete, 01.2019 This product is an autoclaved fibre cement panel
(PCR checked and approved by the SVR) produced by ETEX at Akmene factory in Lithuania and
sold in Europe.
Issue date
31.10.2022 The owner of the declaration shall be liable for the
underlying information and evidence; the IBU shall not
be liable with respect to manufacturer information, life
Valid to
cycle assessment data and evidences.
23.10.2027
The EPD was created according to the specifications
of EN 15804+A2. In the following, the standard will be
simplified as EN 15804.
Verification
The standard EN 15804 serves as the core PCR
Independent verification of the declaration and data
according to ISO 14025:2011
Dipl. Ing. Hans Peters internally x externally
(chairman of Institut Bauen und Umwelt e.V.)
Dr. Alexander Röder Vito D'Incognito
(Managing Director Institut Bauen und Umwelt e.V.)) (Independent verifier)
2. Product
2.1 Product description/Product definition Standard panel thickness 10 mm
Cedral sidings are steam-hardened cellulose- Thermal conductivity 0.212 W/(mK)
reinforced fibre cement panels. They exist in two Flexural strength parallel 23 N/mm2
finishes: smooth or structured (wood relief). Panels are Flexural strength perpendicular 11 N/mm^2
coated and available in various colours. Modulus of elasticity parallel 4000 N/mm2
The manufacturer can - within the framework of the Modulus of elasticity perpendicular 5500 N/mm^2
European Regulation N° 305/2011 (CPR) - present the
Coefficient of thermal expansion <0.01 10-6K-1
Declaration of Performance (DOP) of the product
Swelling (air-dry to water-saturated)
confirming that the product has a CE marking 1.75 mm/m
Hygric movement
2.2 Application
Category
Cedral sidings are used as board-like façade cladding Durability classification EN12467 -
A
for back-ventilated façades. Cedral sidings come as
Strength classification EN12467 Class 2
Cedral Click or Cedral Lap. This EPD only considers
Cedral Lap, as Cedral Click is not produced in
Akmene. The “lap” application foresees an overlap of
For the use and application of the product the
the panels. Once installed correctly according to the
respective (national) provisions at the place of use
manufacturer’s guidelines Cedral needs no further
apply: European standard EN 12467:2012 + A1:2016 +
maintenance, repair, replacement or refurbishment
A2:2006 ‘Fibre-cement flat sheets’.
during the full life span of the product.
2.4 Delivery status
2.3 Technical Data
The products are packed: pallet, PE cover foil,
The following tables include technical data specific to
Coverage carton, PE plastic foam layers and PE band.
the Cedral sidings.
The sheets have the following dimensions:
Constructional data
 Thickness: 10 mm
Name Value Unit
Gross density 1300 kg/m3
2 Environmental Product Declaration Etex – Cedral Sidings
 Cedral classic (length x width): 190 mm x 2.8 Product processing/Installation
3600 mm Description of the type of processing,
machinery and tools used, dust extraction etc.,
 Cedral smooth (length x width): 190 mm x
auxiliary materials needed for installation as well as
3600 mm
measures for noise reduction.
Information on the rules of technology as well as on
workers safety and environmental protection is
2.5 Base materials/Ancillary materials possible.
Base materials included in the composition of Cedral
sidings are: 2.9 Packaging
 Sand: 45-55 % A wooden pallet, PE cover foil, coverage carton, PE
plastic foam layers and PE band are used to pack and
 Cement: 25-35 %
transport the Cedral sidings to the installation site.
 Cellulose: <10 %
 Additives: <3 %
 Coating: <3 % 2.10 Condition of use
 Water: 10-20 % Maintenance requirement will depend on the specific
design and application. Usually, Cedral sidings won’t
change the composition of the materials and thus no
maintenance is needed.
This product/article/at least one partial article contains
substances listed in the candidate list (date:
2.11 Environment and health during use
10.10.2022) exceeding 0.1 percentage by mass: no.
Under normal conditions of use, Cedral sidings do not
cause any adverse health effects or release of volatile
This product/article/at least one partial article contains
organic compounds (VOCs) into indoor air.
other CMR substances in categories 1A or 1B which
No environmental impact on water, air or soil is
are not on the candidate list, exceeding 0.1 percentage
expected due to the extremely low metal release from
by mass: no
the low maintenance requirements.
Biocide products were added to this construction
2.12 Reference service life
product or it has been treated with biocide products
The RSL of the Cedral sidings are estimated at 60
(this then concerns a treated product as defined by the
years.
(EU) Ordinance on Biocide Products No. 528/2012): no
Justification for this assumption: Cedral sidings are a
rather new product on the market (°2007), and there is
not yet extensive evidence regarding its reference
service life. However, there are some studies that
2.6 Manufacture
suggest that it is feasible to assume that this product
Cedral sidings are manufactured largely in accordance
lasts for the average lifetime of a building.[1]
with an automated winding process: the raw materials
The RSL is valid under normal conditions of use.
are mixed with water to prepare a homogenous
mixture. Rotating screen cylinders are immersed in this
[1] Durability of Autoclaved Cellulose Fiber Cement
fibre cement pulp which drain internally. The screen
Composites”, A.M.Cooke, Managing Director, Building
surface is covered in a thin film of fibre cement which
Materials and Technology Pty Ltd, Sydney, NSW,
is transferred onto an infinite conveyor belt from where
Australia
it is conveyed to a format roller which is gradually
https://www.nachhaltigesbauen.de/fileadmin/pdf/baust
covered in an increasingly thicker layer of fibre cement.
off_gebauededaten/BNB_Nutzungsdauern_von_Bautei
Once the requisite material thickness is achieved, the
len__2011-11-03.pdf
still moist and malleable fibre cement layer (fibre
cement fleece) is separated and removed from the
format roller. The fibres cement fleece is cut to size.
2.13 Extraordinary effects
Leftovers are returned to the production process
preventing any waste from being incurred. The panels
Fire
are then set aside for curing before stacking on pallets
and steam-hardened in an autoclave for approx. two
hours. The setting time lasts approx. three days.
Fire protection
Waste from damaged or broken panels is recycled by
Name Value
an external company as raw material for cement
Building material class A2
production. Finally the façade panels are coated in
Burning droplets d0
acrylic paint.
Smoke gas development s1
2.7 Environment and health during
Water
manufacturing
Tests on the product performance including possible
Environmental, occupational health, safety and quality
impacts on the environment following the
management at the Akmene plant are in accordance
unforeseeable influence of water, e.g. flooding showed
with the following standards:
that no risks are expected to occur in terms of
 ISO 14001;2015
environment and human health.
 ISO 9001;2015
 ISO 45001:2018 Mechanical destruction
In case of mechanical destruction, no risks are
3 Environmental Product Declaration Etex – Cedral Sidings
expected to occur in terms of environment and human Scenario A: 100 % landfill
health. Scenario B: While studies (LUBW, 2017) showed that
Cedral sidings can be re-used and recycled, the
2.14 Re-use phase current EPD includes a second end-of-life scenario in
Cedral sidings will be disassembled at the end of its which 100 % of the fibre cement boards are recycled
reference life service (RLS), which is 60 years. (7 % is recycled in cement clinker and 93 % as backfill
The boards are only held in the walls with screws. The in screed). Sidings are designed for recyclability and
disassembly only requires the removal of the screws. are already being recycled in the plant at Kapelle-op-
The same energy as at the installation is necessary for den-Bos (Belgium).
this process.
2.16 Further information
2.15 Disposal Additional information on Cedral sidings can be found
Two end-of-life scenario have been calculated. at: https://www.cedral.world/en/
3. LCA: Calculation rules
3.1 Declared Unit 3.5 Background data
Covering 1 m2 of wall with Cedral sidings, over a The life cycle assesment was done using the LCA
reference service life of 60 years. software package “SimaPro 9.3.0.3” (PRé Consultants,
2021)” in combination with a specific LCA software for
Declared unit ETEX. The main LCA database used in the study is
Name Value Unit the Ecoinvent v3.6 database (September 2019). For
Declared unit 1 m^2 some materials the ELCD or Industry 2.0 database has
Area density 19.5 kg/m^2 been used as no data was available in Ecoinvent or
because these databases better describe the
respective material.
3.2 System boundary 3.6 Data quality
An estimate should be made as regards data quality
This is a cradle-to-grave EPD for the Cedral sidings (addressing both foreground and background data),
with the following life cycle stages included: A1, A2, whereby the age of background data used must be
A3, A4, A5, B1-7, C1, C2, C3, C4 and D. indicated.
For A1, A2 and A3 specific quantities and distances
were collected by ETEX NV and processed by For average EPDs, an estimate of the robustness of
Enperas. For transportation the default capacity the LCA values must be made, e.g. concerning
utilisation factor of the transportation datasets was variability of the production process, geographical
used, as all transportations were mass-based. representatively and the influence of background data
and preliminary products compared to the
3.3 Estimates and assumptions environmental impacts caused by the actual
All assumptions made and the limitations of the LCA production.
study are commented in the report. The results of the
LCA are interpreted in agreement with the goal and 3.7 Period under review
scope and therefore with the ISO 14040 and ISO Data were collected for 2020 for the production
14044 guidelines. process of Cedral sidings in Akmene, Lithuania.
3.4 Cut-off criteria 3.8 Allocation
The following processes are considered below cut-off: At ETEX, different types of fibre cement boards are
 Wearable sieves and cutting knives produced. Only facility level data were available for the
use of electricity, natural gas, propane and water. The
 Transport of packaging of raw material
facility-level data have been allocated to the individual
 Infrastructure and land use of the factory
product using the annual production volume of the
 Packaging and transport of ancillary materials products materials (physical relationship). Material
used during installation inputs and outputs which were not available at the
 Waste treatment of ancillary materials used product level, such as waste, were allocated similarly.
during installation
EN15804+A2 also describes the rules for joint co-
 Environmental impacts caused by the
production, where the processes cannot be divided.
personnel of the production plants are not
The production waste is partly externally recycled.
included in the LCA, e.g. waste from the However, it has been assumed that the recycled waste
cafeteria and sanitary installations, accidental has no economic value, so 100 % of the impacts of the
pollution caused by human mistakes, or production are allocated to the product and 0 % to
environmental effects caused by commuter recycled production waste.
traffic. Heating or cooling of the plants in
3.9 Comparability
order to ensure a comfortable indoor climate
Basically, a comparison or an evaluation of EPD data
for the personnel for example is also
is only possible if all the data sets to be compared
neglected. were created according to EN 15804 and the building
context, respectively the product-specific
characteristics of performance, are taken into account.
4 Environmental Product Declaration Etex – Cedral Sidings
The main LCA database used in the study is the used as no data was available in Ecoinvent or because
Ecoinvent v3.6 database (September 2019). For some these databases better describe the respective
materials, the European Reference Life Cycle material.
Database (ELCD) or Industry 2.0 database has been
4. LCA: Scenarios and additional technical information
Characteristic product properties fix the Cedral sidings. So in total 0,022 kWh of
Information on biogenic carbon electricity is declared.
The product contains biogenic carbon in the form of During the installation, depending on how the Cedral
cellulose. Its accompanying packaging contains sheets are cut, there is a loss rate, depending on the
biogenic carbon in the form of wooden pallets and building shape. For this EPD an average loss rate of 5
carton. Note: 1 kg biogenic Carbon is equivalent to % is used.
44/12 kg of CO .
2
All packaging material for the Cedral sidings is
Information on describing the biogenic Carbon
transported to End of Life (EoL) and disposed of in line
Content at factory gate
with the default EoL scenarios for Germany described
Name Value Unit
in Annexe C of the Product Environmental Footprint
Biogenic Carbon Content in product 0.47 kg C
Pilots (PEFCR) 6.3 guidance.
Biogenic Carbon Content in
0.469 kg C
accompanying packaging
The packaging of the ancillary materials used during
installation are considered below cut-off.
Name Value Unit
Transport to the building site (A4) Auxiliary Inox screws 0.038 kg
The following transport scenario has been used to Electricity consumption To fix the
0.022 kWh
model the transport from the manufacturing plant in screws
Akmene (Lithuania) to the installation site in Europe. Material loss 5 %
Packaging
- 29 % directly to the construction site over 709 km final
with a 16-32 ton lorry (ecoinvent record: ‘Transport, product:
freight, lorry 16-32 metric ton, EURO5 {RER}| wooden
transport, freight, lorry 16-32 metric ton, EURO5 | Cut- pallet, PE-
off, U’ Output substances following band, PE
waste treatment on site cover foil,
- 71 % to a supplier over 1274 km with a >32 ton lorry PE plastic
(ecoinvent record: ‘Transport, freight, lorry >32 metric foam
ton, EURO5 {RER}| transport, freight, lorry >32 metric layers,
ton, EURO5 | Cut-off, U’) and from the supplier to the coverage
installation site over 35 km with a 16-32 ton lorry carton
(ecoinvent record: ‘Transport, freight, lorry 16-32
metric ton, EURO5 {RER}| transport, freight, lorry 16-
32 metric ton, EURO5 | Cut-off, U’)
Use phase B1-7
Losses during transport are considered during the
Over the 60 years of reference service life (RSL), if
installation phase, as it is difficult to separately quantify
correctly installed, there are no impacts for the use
the specific transport and installation losses.
phase (B1-7), except for the carbonation in module B1.
The calculations for the carbonation are described in
Name Value Unit section 5.
Litres of fuel 25.6 l/100km Name Value Unit
Transport distance (29 % directly
709 km
to construction site) Maintenance (B2)
Transport distance (71 % to a The product does not require maintenance.
1274 km
supplier) Name Value Unit
Transport distance (71 % from
35 km
supplier to construction site) Repair (B3)
Capacity utilisation (including The product does not require repair.
50 %
empty runs) Name Value Unit
Gross density of products Scenario
transported Ecoinvent kg/m3 Replacement (B4) / Refurbishment (B5)
No replacement/refurbishment required.
Scenario
Capacity utilisation volume factor Ecoinvent - Name Value Unit
Installation into the building (A5)
Reference service life
12.5 inox screws (or 0.038 kg) are necessary per
Name Value Unit
functional unit for Cedral sidings. The installation
Life Span according to the
involves an amount of 0.00176 kWh per screw used to 60 a
manufacturer
5 Environmental Product Declaration Etex – Cedral Sidings
Design application parameters (if Following waste streams are considered after their
instructed by the manufacturer), end-of-waste point in this study: steel screws in C3 (of
including the references to the - - which 95 % are recycled), wooden pallets in A3 and A5
appropriate practices and application (of which 30 % are recycled and respectively 7 % and
codes 32 % are incinerated with efficiency <60 %), plastic
An assumed quality of work, when packaging in A3 and A5 (of which respectively 27 %
installed in accordance with the - - and 29 % are recycled and respectively 27 % and 32
manufacturer’s instructions % are incinerated with efficiency <60 %), paper and
Outdoor environment, (for outdoor cardboard in A3 and A5 (of which 75 % are recycled
applications), e.g. weathering, and respectively 3 % and 11 % are incinerated), and
pollutants, UV and wind exposure, - - steel cables in A3 (of which respectively 95 % are
building orientation, shading, recycled).
temperature
Indoor environment (for indoor For the additional end-of-life scenario (Scenario B),
applications), e.g. temperature, - - 100 % of the fiber cement boards are recycled and
moisture, chemical exposure reaches the end-of-waste state. This is taken into
Usage conditions, e.g. frequency of account in module D of Scenario B.
- -
use, mechanical exposure Name Value Unit
Quantitative description of the loads
Maintenance e.g. required frequency,
beyond the system boundaries
type and quality and replacement of - -
Treatment of scrap steel to prepare it 0.039 kg
components
for to prepare it for recycling at the
remelter
Operational energy use (B6) and Operational water
Quantitative description of the benefits
use (B7)
beyond the system boundaries Sorting
The product does not require operational energy/water 0.313 kg
of waste wood to prepare it for
use.
recycling
Name Value Unit
Quantitative description of the benefits
End of life (C1-C4) beyond the system boundaries
0.061 kg
The dismantling of Cedral sidings involves the same Treatment kg plastic to prepare it for
amount of energy as for the installation, which is 0,022 recycling
kWh. Quantitative description of the benefits
beyond the system boundaries
1.51 MJ
In module C2, the impacts due to the transport of Avoided production of heat using
waste from the final product to waste processing are natural gas
calculated. Quantitative description of the benefits
- to recycling - 200 km beyond the system boundaries
0.75 MJ
- to incineration - 150 km Avoided production of European
- to landfill - 50 km electricity mix
Quantitative description of the benefits
Two end-of-life scenarios have been calculated. beyond the system boundaries 0.039 kg
Scenario A: 100 % of the fibre cement board and 5 % Avoided production of primary steel
of the steel screws are landfilled, The end-of-waste Quantitative description of the benefits
state is not reached. 95 % of the steel screws are beyond the system boundaries
0.313 kg
recycled at their end of life. The end-of-waste state is Avoided production of primary
reached after the sorting. softwood
Scenario B: While studies showed that Cedral sidings Quantitative description of the benefits
can be re-used and recycled, the current EPD includes beyond the system boundaries
a second end-of-life scenario in which 100 % of the Avoided production of primary 0.061 kg
fibre cement boards are recycled (7 % is recycled in polypropylene/polypropylene
cement clinker and 93 % as backfill in screed) and 95 granulates
% of the steel screws are recycled. The end end-of- Quantitative description of the benefits
waste state is reached after sorting. 5 % of the steel beyond the system boundaries (only
1.635 kg
screws are landfilled. The end-of-waste state is not EoL scenario B) Avoided production of
reached. primary limestone
Quantitative description of the benefits
Name Value Unit beyond the system boundaries (only
18.135 kg
Collected separately waste type 19.538 kg EoL scenario B) Avoided production of
Collected as mixed construction waste 0 kg primary sand
Reuse 0 kg
Reuse (Scenario B) 0 kg
Recycling 0.036 kg
Recycling (Scenario B) 19.536 kg
Energy recovery 0 kg
Energy recovery (Scenario B) 0 kg
Landfilling 19.502 kg
Landfill (Scenario B) 0.002 kg
Reuse, recovery and/or recycling potentials (D),
relevant scenario information
6 Environmental Product Declaration Etex – Cedral Sidings
5. LCA: Results
While studies [2] showed that Cedral sidings can be reused and recycled, the current EPD assumes 100 %
landfilling of the product at its end of life.
Sidings are designed for recyclability and are already being recycled in the plant at Kapelle-op-den-Bos
(Belgium). The waste of the fibre cement and calcium silicate boards (both pre- and post-consumer waste), will no
longer go to landfill: 7 % in cement clinker and 93 % as backfill in screed. Therefore, also a 100 % recycling
scenario has been calculated and included in the results (see columns C2/1, C3/1, C4/1 and D/1 in the results
tables).
[2] Landesanstalt für Umwelt, Messungen und Naturschutz Baden -Württemberg, Steckbrief „Asbestfreie
Faserzementprodukte“
Note that the effect of carbonation has been included in module B1. Using the formula below a CO uptake of
2
1.93 kgCO eq due to carbonation during the use phase is calculated
2
Carbonation = Dc x Qcem x %Ccem x 0.65 x m.m CO /m.m CaO
2
 m.mCO = molecular mass of CO
2 2
 m.m CaO = molecular mass of CaO
 0.65 = % of CaO in cement clinker
 Qcem= amount of cement used for producing 1m² of Cedral sidings
 %Ccem = percentage of clinker in cement which is at least 90 % in Portland cement (used in Cedral
siding) according to EN16757
 Dc = degree of carbonation according to EN16757 whereas Dc will depend on the exposure conditions.
75 % has been assumed.
DESCRIPTION OF THE SYSTEM BOUNDARY (X = INCLUDED IN LCA; ND = MODULE OR INDICATOR NOT
DECLARED; MNR = MODULE NOT RELEVANT)
BENEFITS AND
CONSTRUCTI LOADS
PRODUCT STAGE ON PROCESS USE STAGE END OF LIFE STAGE BEYOND THE
STAGE SYSTEM
BOUNDARIES
7 Environmental Product Declaration Etex – Cedral Sidings
lairetam
waR
ylppus tropsnarT
gnirutcafunaM
eht
morf
tropsnarT
etis
eht
ot
etag
ylbmessA esU
ecnanetniaM
riapeR
tnemecalpeR tnemhsibrufeR
ygrene
lanoitarepO esu
retaw
lanoitarepO esu
noitcurtsnoc-eD
noitilomed tropsnarT
gnissecorp
etsaW
lasopsiD -esueR -yrevoceR -gnilcyceR laitnetop
A1 A2 A3 A4 A5 B1 B2 B3 B4 B5 B6 B7 C1 C2 C3 C4 D
X X X X X X X X X X X X X X X X X
RESULTS OF THE LCA - ENVIRONMENTAL IMPACT according to EN 15804+A2: 1 m^2 wall covered with
Cedral sidings
Core Indicator Unit A1 A2 A3 A4 A5 B1 B2 B3 B4 B5 B6 B7 C1 C2 C2/1 C3 C3/1 C4 C4/1 D D/1
- - -
4.01E1.01E4.20E2.55E2.89E 0.00E0.00E0.00E0.00E0.00E0.00E9.53E1.73E8.23E1.66E1.77E1.85E4.33E
GWP-total [kg CO2-Eq.]
+0 +0 -1 +0 +0
1.93E
+0 +0 +0 +0 +0 +0 -3 -1 -1 -4 +0 +0 -5
5.23E2.29E
+0 -1 +0
- -
5.77E1.01E2.04E2.55E1.17E0.00E0.00E0.00E0.00E0.00E0.00E0.00E9.44E1.73E8.22E1.63E4.85E1.32E4.29E
GWP-fossil [kg CO2-Eq.]
+0 +0 +0 +0 +0 +0 +0 +0 +0 +0 +0 +0 -3 -1 -1 -4 -2 -1 -5
5.23E5.67E
-1 -1
- - -
3.93E 1.05E1.72E0.00E0.00E0.00E0.00E0.00E0.00E0.00E6.61E7.04E3.35E2.70E1.72E1.72E4.17E6.67E
GWP-biogenic [kg CO2-Eq.] 1.77E
-4
1.62E
-3 +0 +0 +0 +0 +0 +0 +0 +0 -5 -5 -4 -6 +0 +0 -7 -4
1.72E
+0 +0 +0
- -
2.19E4.03E2.36E7.93E5.90E0.00E0.00E0.00E0.00E0.00E0.00E0.00E2.20E6.03E2.87E1.94E5.12E6.74E2.20E
GWP-luluc [kg CO2-Eq.]
-3 -4 -3 -4 -4 +0 +0 +0 +0 +0 +0 +0 -5 -5 -4 -7 -5 -5 -8
6.99E7.28E
-4 -4
- -
2.53E2.26E2.69E5.93E9.73E0.00E0.00E0.00E0.00E0.00E0.00E0.00E7.95E3.92E1.87E6.59E3.03E4.37E9.31E
ODP [kg CFC11-Eq.] 4.65E5.46E
-7 -7 -7 -7 -8 +0 +0 +0 +0 +0 +0 +0 -10 -8 -7 -12 -9 -8 -12
-8 -8
- -
1.74E8.24E8.55E1.06E4.25E0.00E0.00E0.00E0.00E0.00E0.00E0.00E5.51E7.05E3.36E4.86E1.90E1.01E2.61E
AP [mol H+-Eq.] 1.98E2.43E
-2 -3 -3 -2 -3 +0 +0 +0 +0 +0 +0 +0 -5 -4 -3 -7 -4 -3 -7
-3 -3
- -
9.74E7.43E5.19E1.96E2.11E0.00E0.00E0.00E0.00E0.00E0.00E0.00E1.01E1.36E6.46E2.43E6.37E6.97E1.91E
EP-freshwater [kg P-Eq.] 2.20E2.31E
-5 -6 -5 -5 -5 +0 +0 +0 +0 +0 +0 +0 -6 -6 -6 -8 -6 -6 -9
-5 -5
- -
4.19E2.20E2.71E3.18E1.06E0.00E0.00E0.00E0.00E0.00E0.00E0.00E6.99E2.09E9.97E7.83E4.84E3.54E8.00E
EP-marine [kg N-Eq.] 3.88E5.43E
-3 -3 -3 -3 -3 +0 +0 +0 +0 +0 +0 +0 -6 -4 -4 -8 -5 -4 -8
-4 -4
- -
4.87E2.44E2.98E3.52E1.18E0.00E0.00E0.00E0.00E0.00E0.00E0.00E8.62E2.31E1.10E1.21E6.22E3.99E9.01E
EP-terrestrial [mol N-Eq.] 4.41E6.29E
-2 -2 -2 -2 -2 +0 +0 +0 +0 +0 +0 +0 -5 -3 -2 -6 -4 -3 -7
-3 -3
- -
1.29E6.88E1.03E1.11E3.50E0.00E0.00E0.00E0.00E0.00E0.00E0.00E2.19E7.09E3.38E2.40E1.47E1.11E2.75E
POCP [kg NMVOC-Eq.] 1.67E2.15E
-2 -3 -2 -2 -3 +0 +0 +0 +0 +0 +0 +0 -5 -4 -3 -7 -4 -3 -7
-3 -3
- -
3.35E1.80E2.83E3.73E6.42E0.00E0.00E0.00E0.00E0.00E0.00E0.00E1.29E3.36E1.60E2.73E7.28E1.31E7.04E
ADPE [kg Sb-Eq.] 5.13E6.87E
-6 -6 -6 -6 -6 +0 +0 +0 +0 +0 +0 +0 -8 -7 -6 -10 -8 -7 -11
-7 -7
- -
3.84E1.49E4.32E3.93E1.08E0.00E0.00E0.00E0.00E0.00E0.00E0.00E1.94E2.60E1.24E2.21E6.59E3.35E7.99E
ADPF [MJ] 1.05E1.13E
+1 +1 +1 +1 +1 +0 +0 +0 +0 +0 +0 +0 -1 +0 +1 -3 -1 +0 -4
+1 +1
- - -
[m³ world-Eq 2.20E3.92E1.32E1.22E2.32E0.00E0.00E0.00E0.00E0.00E0.00E0.00E2.18E7.24E3.45E8.65E2.37E1.05E
WDP 2.22E1.32E1.71E
deprived] +0 -2 +0 -1 -1 +0 +0 +0 +0 +0 +0 +0 -3 -3 -2 -6 -3 -2
-5 -1 -1
GWP = Global warming potential; ODP = Depletion potential of the stratospheric ozone layer; AP = Acidification potential of land and water; EP =
Caption Eutrophication potential; POCP = Formation potential of tropospheric ozone photochemical oxidants; ADPE = Abiotic depletion potential for non-
fossil resources; ADPF = Abiotic depletion potential for fossil resources; WDP = Water (user) deprivation potential
RESULTS OF THE LCA - INDICATORS TO DESCRIBE RESOURCE USE according to EN 15804+A2: 1 m^2
wall covered with Cedral sidings
Indicator Unit A1 A2 A3 A4 A5 B1 B2 B3 B4 B5 B6 B7 C1 C2 C2/1 C3 C3/1 C4 C4/1 D D/1
2.27E1.92E2.91E5.04E8.06E0.00E0.00E0.00E0.00E0.00E0.00E0.00E3.63E3.60E1.71E3.94E1.03E1.43E3.16E0.00E0.00E
PERE [MJ]
+1 -1 +1 -1 +0 +0 +0 +0 +0 +0 +0 +0 -2 -2 -1 -4 -1 -1 -5 +0 +0
- -
1.54E0.00E1.43E0.00E 0.00E0.00E0.00E0.00E0.00E0.00E0.00E0.00E0.00E0.00E0.00E 0.00E0.00E4.60E1.98E
PERM [MJ] 7.70E 1.52E
+1 +0 +1 +0 +0 +0 +0 +0 +0 +0 +0 +0 +0 +0 +0 +0 +0 +0 +1
+0 +1
-
3.81E1.92E4.35E5.04E3.60E0.00E0.00E0.00E0.00E0.00E0.00E0.00E3.63E3.60E1.71E3.94E 1.43E3.16E4.60E1.98E
PERT [MJ] 1.51E
+1 -1 +1 -1 -1 +0 +0 +0 +0 +0 +0 +0 -2 -2 -1 -4 -1 -5 +0 +1
+1
4.30E1.50E3.72E3.95E1.44E0.00E0.00E0.00E0.00E0.00E0.00E0.00E2.33E2.62E1.25E2.97E8.58E3.53E8.68E0.00E0.00E
PENRE [MJ]
+1 +1 +1 +1 +1 +0 +0 +0 +0 +0 +0 +0 -1 +0 +1 -3 -1 +0 -4 +0 +0
-
5.55E0.00E8.92E0.00E 0.00E0.00E0.00E0.00E0.00E0.00E0.00E0.00E0.00E0.00E0.00E0.00E0.00E0.00E1.48E1.48E
PENRM [MJ] 2.41E
-2 +0 +0 +0 +0 +0 +0 +0 +0 +0 +0 +0 +0 +0 +0 +0 +0 +0 -2 -2
+0
4.31E1.50E4.61E3.95E1.20E0.00E0.00E0.00E0.00E0.00E0.00E0.00E2.33E2.62E1.25E2.97E8.58E3.53E8.68E1.48E1.48E
PENRT [MJ]
+1 +1 +1 +1 +1 +0 +0 +0 +0 +0 +0 +0 -1 +0 +1 -3 -1 +0 -4 -2 -2
1.13E0.00E0.00E0.00E0.00E0.00E0.00E0.00E0.00E0.00E0.00E0.00E0.00E0.00E0.00E0.00E0.00E0.00E0.00E9.48E2.14E
SM [kg]
-3 +0 +0 +0 +0 +0 +0 +0 +0 +0 +0 +0 +0 +0 +0 +0 +0 +0 +0 -1 +1
0.00E0.00E0.00E0.00E0.00E0.00E0.00E0.00E0.00E0.00E0.00E0.00E0.00E0.00E0.00E0.00E0.00E0.00E0.00E0.00E0.00E
RSF [MJ]
+0 +0 +0 +0 +0 +0 +0 +0 +0 +0 +0 +0 +0 +0 +0 +0 +0 +0 +0 +0 +0
0.00E0.00E0.00E0.00E0.00E0.00E0.00E0.00E0.00E0.00E0.00E0.00E0.00E0.00E0.00E0.00E0.00E0.00E0.00E0.00E0.00E
NRSF [MJ]
+0 +0 +0 +0 +0 +0 +0 +0 +0 +0 +0 +0 +0 +0 +0 +0 +0 +0 +0 +0 +0
- - -
1.40E1.00E3.17E3.06E1.06E0.00E0.00E0.00E0.00E0.00E0.00E0.00E1.43E1.88E8.96E6.53E1.73E3.34E
FW [m³] 5.09E3.41E2.91E
-1 -3 -2 -3 -2 +0 +0 +0 +0 +0 +0 +0 -4 -4 -4 -7 -4 -3
-7 -3 -2
PERE = Use of renewable primary energy excluding renewable primary energy resources used as raw materials; PERM = Use of
renewable primary energy resources used as raw materials; PERT = Total use of renewable primary energy resources; PENRE = Use of
non-renewable primary energy excluding non-renewable primary energy resources used as raw materials; PENRM = Use of non-
Caption
renewable primary energy resources used as raw materials; PENRT = Total use of non-renewable primary energy resources; SM = Use
of secondary material; RSF = Use of renewable secondary fuels; NRSF = Use of non-renewable secondary fuels; FW = Use of net fresh
water
RESULTS OF THE LCA – WASTE CATEGORIES AND OUTPUT FLOWS according to EN 15804+A2:
1 m^2 wall covered with Cedral sidings
8 Environmental Product Declaration Etex – Cedral Sidings
Indicator Unit A1 A2 A3 A4 A5 B1 B2 B3 B4 B5 B6 B7 C1 C2 C2/1 C3 C3/1 C4 C4/1 D D/1
- -
3.29E3.59E6.23E9.77E1.90E0.00E0.00E0.00E0.00E0.00E0.00E0.00E1.30E6.82E3.25E2.90E9.83E3.98E1.53E
HWD [kg] 1.78E1.97E
-5 -5 -5 -5 -5 +0 +0 +0 +0 +0 +0 +0 -7 -6 -5 -9 -7 -6 -9
-5 -5
- -
3.62E6.29E2.01E2.92E1.79E0.00E0.00E0.00E0.00E0.00E0.00E0.00E6.87E1.25E5.93E9.86E2.67E1.95E2.84E
NHWD [kg] 4.00E4.54E
-1 -1 -1 +0 +0 +0 +0 +0 +0 +0 +0 +0 -4 -1 -1 -6 -3 +1 -3
-2 -2
- -
1.31E1.02E7.67E2.68E4.51E0.00E0.00E0.00E0.00E0.00E0.00E0.00E1.38E1.78E8.45E8.91E2.90E2.12E4.47E
RWD [kg] 2.61E3.19E
-4 -4 -5 -4 -5 +0 +0 +0 +0 +0 +0 +0 -6 -5 -5 -9 -6 -5 -9
-5 -5
0.00E0.00E0.00E0.00E0.00E0.00E0.00E0.00E0.00E0.00E0.00E0.00E0.00E0.00E0.00E0.00E0.00E0.00E0.00E0.00E0.00E
CRU [kg]
+0 +0 +0 +0 +0 +0 +0 +0 +0 +0 +0 +0 +0 +0 +0 +0 +0 +0 +0 +0 +0
- -
0.00E0.00E5.38E0.00E4.11E0.00E0.00E0.00E0.00E0.00E0.00E0.00E0.00E0.00E0.00E0.00E1.95E0.00E0.00E
MFR [kg] 9.49E2.14E
+0 +0 -1 +0 -1 +0 +0 +0 +0 +0 +0 +0 +0 +0 +0 +0 +1 +0 +0
-1 +1
0.00E0.00E0.00E0.00E0.00E0.00E0.00E0.00E0.00E0.00E0.00E0.00E0.00E0.00E0.00E0.00E0.00E0.00E0.00E0.00E0.00E
MER [kg]
+0 +0 +0 +0 +0 +0 +0 +0 +0 +0 +0 +0 +0 +0 +0 +0 +0 +0 +0 +0 +0
- -
0.00E0.00E2.59E0.00E7.52E0.00E0.00E0.00E0.00E0.00E0.00E0.00E0.00E0.00E0.00E0.00E0.00E0.00E0.00E
EEE [MJ] 7.55E7.55E
+0 +0 -3 +0 -1 +0 +0 +0 +0 +0 +0 +0 +0 +0 +0 +0 +0 +0 +0
-1 -1
- -
0.00E0.00E5.19E0.00E1.50E0.00E0.00E0.00E0.00E0.00E0.00E0.00E0.00E0.00E0.00E0.00E0.00E0.00E0.00E
EET [MJ] 1.51E1.51E
+0 +0 -3 +0 +0 +0 +0 +0 +0 +0 +0 +0 +0 +0 +0 +0 +0 +0 +0
+0 +0
HWD = Hazardous waste disposed; NHWD = Non-hazardous waste disposed; RWD = Radioactive waste disposed; CRU = Components
Caption for re-use; MFR = Materials for recycling; MER = Materials for energy recovery; EEE = Exported electrical energy; EET = Exported
thermal energy
RESULTS OF THE LCA – additional impact categories according to EN 15804+A2-optional:
1 m^2 wall covered with Cedral sidings
Indicator Unit A1 A2 A3 A4 A5 B1 B2 B3 B4 B5 B6 B7 C1 C2 C2/1 C3 C3/1 C4 C4/1 D D/1
- -
[Disease 1.55E6.47E1.81E2.13E5.64E0.00E0.00E0.00E0.00E0.00E0.00E0.00E1.44E1.20E5.72E2.23E2.26E1.96E7.99E
PM 1.83E2.73E
Incidence] -7 -8 -7 -7 -8 +0 +0 +0 +0 +0 +0 +0 -10 -8 -8 -12 -9 -8 -12
-8 -8
- -
[kBq U235-1.46E6.49E7.45E1.72E3.85E0.00E0.00E0.00E0.00E0.00E0.00E0.00E1.68E1.14E5.42E6.94E2.17E1.39E2.95E
IRP 2.84E3.49E
Eq.] -1 -2 -2 -1 -2 +0 +0 +0 +0 +0 +0 +0 -3 -2 -2 -6 -3 -2 -6
-2 -2
- -
5.94E1.17E3.06E3.13E1.60E0.00E0.00E0.00E0.00E0.00E0.00E0.00E1.33E2.08E9.93E1.90E5.47E2.03E1.52E
ETP-fw [CTUe] 6.01E9.81E
+1 +1 +1 +1 +1 +0 +0 +0 +0 +0 +0 +0 -1 +0 +0 -3 -1 +0 -3
+0 +0
- -
2.47E3.76E1.54E8.07E4.01E0.00E0.00E0.00E0.00E0.00E0.00E0.00E3.44E5.86E2.79E5.93E1.72E4.85E8.70E
HTP-c [CTUh] 6.02E6.52E
-9 -10 -9 -10 -9 +0 +0 +0 +0 +0 +0 +0 -12 -11 -10 -14 -11 -11 -14
-10 -10
- -
6.32E1.24E2.49E3.52E1.99E0.00E0.00E0.00E0.00E0.00E0.00E0.00E1.17E2.27E1.08E1.75E5.00E1.31E1.06E
HTP-nc [CTUh] 6.15E7.09E
-8 -8 -8 -8 -8 +0 +0 +0 +0 +0 +0 +0 -10 -9 -8 -12 -10 -9 -12
-9 -9
- -
1.44E9.25E2.36E3.92E2.40E0.00E0.00E0.00E0.00E0.00E0.00E0.00E4.75E1.79E8.55E1.65E4.40E6.38E1.18E
SQP [-] 8.25E8.37E
+2 +0 +2 +1 +1 +0 +0 +0 +0 +0 +0 +0 -2 +0 +0 -3 -1 +0 -3
+1 +1
PM = Potential incidence of disease due to PM emissions; IR = Potential Human exposure efficiency relative to U235; ETP-fw = Potential
Caption comparative Toxic Unit for ecosystems; HTP-c = Potential comparative Toxic Unit for humans (cancerogenic); HTP-nc = Potential
comparative Toxic Unit for humans (not cancerogenic); SQP = Potential soil quality index
6. LCA: Interpretation
The results show the contribution of the various steps impact category. Outside the system boundaries,
in the life cycle, per environmental impact category, for module D shows benefits from the energy recovery
1 m2 of Cedral sidings produced in Akmene. Te raw and recycling processes which are related to
materials used in the formulation mix have the highest packaging materials for Cedral sidings. For the
contribution on most impact categories followed by the additional end-of-life scenario (Scenario B) module D
transportation of the final product, the production also takes the benefits from recycling of the fiber
process of Cedral siding, the installation and the cement board itself into account.
transport of the raw materials, depending on the
7. Requisite evidence
7.1 Radioactivity 7.3 VOC emissions
Not measured Not applicable as Cedral sidings are designed for
external applications
7.2 Leaching
AgBB overview of results (28 days [µg/m³])
No leaching test was done since 2020 at Akmene due Name Value Unit
to the changed Lithuanian legal acts TVOC (C6 - C16) - μg/m3
Sum SVOC (C16 - C22) - μg/m3
9 Environmental Product Declaration Etex – Cedral Sidings
R (dimensionless) - - TVOC (C6 - C16) - μg/m3
VOC without NIK - μg/m3 Sum SVOC (C16 - C22) - μg/m3
Carcinogenic Substances - μg/m3 R (dimensionless) - -
VOC without NIK - μg/m3
AgBB overview of results (3 days [µg/m³]) Carcinogenic Substances - μg/m3
Name Value Unit
8. References
Standards Pré Consultants (2021) SimaPro 9.2.0.1 [Computer
EN15804 Software]. Amersfoort, The Netherlands.
EN 15804:2012+A2:2019+AC:2021, Sustainability of
construction works — Environmental Product CPR
Declarations — Core rules for the product category of European Regulation N° 305/2011 (CPR)
construction products.
Ecoinvent
PCR Part A Wernet, G., Bauer, C., Steubing, B., Reinhard, J.,
Calculation rules for the Life Cycle Assessment and Moreno-Ruiz, E., and Weidema, B., 2016. The
Requirements on the Background Report, Institut ecoinvent database version 3 (part I): overview and
Bauen und Umwelt e.V., www.bauumwelt.com. methodology. The International Journal of Life Cycle
Assessment, [online] 21(9), pp.1218–1230. Available
PCR Part B at: <http://link.springer.com/10.1007/s11367-016-1087-
Institut Bauen und Umwelt e.V, Berlin (pub.): PCR 8> .
Guidance-Texts for Building-Related Products and
Services From the range of Environmental Product ELCD
Declarations of Institute Construction and Environment European commission (2018). European reference Life
e.V. (IBU) : Requirements on the EPD for Fibre cement Cycle Database v3.2. 2018.
/ Fibre concrete https://eplca.jrc.ec.europa.eu/ELCD3/
EN12467 Industry 2.0
EN 12467:2012 + A1:2016 + A2:2006 ‘Fibre-cement Industry 2.0 (from PlasticsEurope, worldsteel and
flat sheets’ ERASM) LCA database as integrated in SimaPro
9.3.0.3.
EN16757
EN 16757:2017, Sustainability of construction works– PEFCR
Environmental product declarations – Product European commission (2018). Product Environmental
Category Rules for concrete and concrete elements Footprint Category Rules PEFCR Guidance, version
6.3.
ISO 14025
EN ISO 14025:2011, Environmental labels and Reuse and recycling
declarations — Type III environmental declarations — LUBW. Landesanstalt für Umwelt, Messungen und
Principles and procedures. Naturschutz Baden -Württemberg, Steckbrief
„Asbestfreie Faserzementprodukte“. 2017.
ISO 14040 https://www.lubw.baden-
ISO 14040:2006: Environmental management – Life wuerttemberg.de/documents/10184/151537/Steckbrief
cycle assessment – Principles and framework. +25-7_Asbestfreie+Faserzementprodukte_17-10-
10.pdf/f713de93-88f8-4356-b45d-b4804085b9e3
ISO 14044
ISO 14044:2006: Environmental management – Life Durability
cycle assessment – Requirements and guidelines. Durability of Autoclaved Cellulose Fiber Cement
Composites”, A.M.Cooke, Managing Director, Building
ISO 14001 Materials and Technology Pty Ltd, Sydney, NSW,
ISO 14001:2015: Environmental management systems Australia
— Requirements with guidance for use http://www.fibrecementconsulting.com/publications/990
925.durabilitypaper.pdf
ISO 9001
ISO 9001:2015: Quality management systems — IBU
Requirements IBU 2021. Institut Bauen und Umwelt e.V.: General
Instructions for the EPD programme of Institut Bauen
ISO 45001 und Umwelt e.V., Version 2.0, Berlin: Institut Bauen
ISO 45001:2018: Occupational health and safety und Umwelt e.V., 2021 www.ibu-epd.com
management systems Requirements with guidance for
use
Further references
10 Environmental Product Declaration Etex – Cedral Sidings
Publisher
Institut Bauen und Umwelt e.V. Tel +49 (0)30 3087748- 0
Hegelplatz 1 Fax +49 (0)30 3087748- 29
10117 Berlin Mail info@ibu-epd.com
Germany Web www.ibu-epd.com
Programme holder
Institut Bauen und Umwelt e.V. Tel +49 (0)30 - 3087748- 0
Hegelplatz 1 Fax +49 (0)30 – 3087748 - 29
10117 Berlin Mail info@ibu-epd.com
Germany Web www.ibu-epd.com
Author of the Life Cycle
Assessment Tel +32 3 376 00 19
Enperas Fax -
Thorpark 8300 Mail info@enperas.com
3600 Genk Web https://www.enperas.com/en/
Belgium
Owner of the Declaration
Etex Building Performance Tel +32 2 778 12 11
International Fax +32 2 778 12 12
Rue Marcel Demonque 500 Mail info@etexgroup.com
84915 Avignon Cedex 9 Web http://www.etexgroup.com
France
