Environmental Product Declaration (EPD)
According to ISO 14025 and EN 15804
ACEMat™
Registration number: EPD-Kiwa-EE-158056-EN
Issue date: 22-12-2023
Valid until: 22-12-2028
Declaration owner: Gold-Joint Industry Co., Ltd.
Publisher: Kiwa-Ecobility Experts
Program operator: Kiwa-Ecobility Experts
Status: verified
ACEMat™ | ReTHiNK-58056 1 / 24
Environmental Product Declaration
1 General information
E-mail: marketing@geoace.com
1.1 PRODUCT Website: www.geoace.com
Production location: Gold-Joint Industry Co., Ltd.
ACEMat™
Address production location: No.33, Jing 3 Rd. Wuqi Dist., 43541 Taichung City
1.2 REGISTRATION NUMBER
1.6 VERIFICATION OF THE DECLARATION
EPD-Kiwa-EE-158056-EN
The independent verification is in accordance with the ISO 14025:2011. The LCA is in
1.3 VALIDITY compliance with ISO 14040:2006 and ISO 14044:2006. The EN 15804:2012+A2:2019 serves as
the core PCR.
Issue date: 22-12-2023
Internal ✓ External
Valid until: 22-12-2028
1.4 PROGRAM OPERATOR
Kiwa-Ecobility Experts
Voltastraße 5
13355 Berlin
DE
Elisabeth Amat Guasch, Greenize
1.7 STATEMENTS
Prof. Dr. Frank Heimbecher
The owner of this EPD shall be liable for the underlying information and evidence. The
(Chairman of the independent expert
programme operator Kiwa-Ecobility Experts shall not be liable with respect to
committee - Kiwa-Ecobility Experts)
manufacturer data, life cycle assessment data and evidence.
Frank Huppertz 1.8 PRODUCT CATEGORY RULES
(Head of Kiwa-Ecobility Experts)
Kiwa-Ecobility Experts (Kiwa-EE) – General Product Category Rules (2022-02-14)
Kiwa-Ecobility Experts (Kiwa-EE) – Specific Product Category Rules: Geosynthetic products
1.5 OWNER OF THE DECLARATION
(2023-07-21)
Manufacturer: Gold-Joint Industry Co., Ltd.
Address: No.33, Jing 3 Rd. Wuqi Dist., 43541 Taichung City, Taiwan (R.O.C.)
ACEMat™ | ReTHiNK-58056 2 / 24
Environmental Product Declaration
1 General information
1.9 COMPARABILITY 1.10 CALCULATION BASIS
In principle, a comparison or assessment of the environmental impacts of different LCA method R<THiNK: Ecobility Experts | EN15804+A2
products is only possible if they have been prepared in accordance with EN 15804. For the
evaluation of the comparability, the following aspects have to be considered in particular: LCA software*: Simapro 9.1
PCR used, functional or declared unit, geographical reference, the definition of the system Characterization method: EN 15804 +A2 Method v1.0
boundary, declared modules, data selection (primary or secondary data, background
database, data quality), scenarios used for use and disposal phases, and the life cycle LCA database profiles: EcoInvent version 3.6
inventory (data collection, calculation methods, allocations, validity period). PCRs and Version database: v3.15 (2023-07-12)
general program instructions of different EPDs programs may differ. Comparability needs
to be evaluated. For further guidance, see EN 15804+A2 (5.3 Comparability of EPD for
*Used for calculating the characterized results of the Environmental profiles within
construction products) and ISO 14025 (6.7.2 Requirements for comparability).
R<THiNK.
1.11 LCA BACKGROUND REPORT
This EPD is generated on the basis of the LCA background report 'ACEMat™' with the
calculation identifier ReTHiNK-58056.
ACEMat™ | ReTHiNK-58056 3 / 24
Environmental Product Declaration
2 Product
2.1 PRODUCT DESCRIPTION foundations, thus destabilizing slopes. ACEMat™ not only enhances slope filtration and
stabilization but also encourages vegetation growth, offering robust soil and rock slope
erosion resistance.
ACEMat™ is a Turf Reinforcement Mat (TRM) made of high-strength polypropylene
monofilament. With its stable and thick three-dimensional woven structures, ACEMat™ is
In environmental restoration, ACEMat™'s ability to promote vegetation and retain soil
highly effective in controlling severe erosion problems in steep slopes, barren areas,
makes it a key tool, especially given rising concerns over land degradation. Additionally,
riverbanks, channels, and areas with heavy rainfall. It interlocks with soil to create a solid
these mats are used in constructing channels and swales where they reduce erosion and
base, dissipating run-off and stream erosive forces while protecting the soil surface from
support vegetation. Research is underway to evaluate their potential in optimizing
water splash and wash. Furthermore, it retains seeds and supports plants when vegetation
hydraulic efficiency and maintaining channel bed integrity. Their relevance is growing in
is required, providing exceptional erosion control and enhanced vegetation performance.
stormwater management, as they could mitigate runoff and facilitate water infiltration,
contributing to sustainable practices, particularly as climate-related challenges like
increased precipitation become more common.
2.3 REFERENCE SERVICE LIFE
RSL PRODUCT
According to the recommendations of the Erosion Control Technology Council, the
Reference Service Life (RSL) of Rolled Erosion Control Products (RECPs) can be categorized
as temporary, with subdivisions of 3 months, 12 months, 24 months, and 36 months, and
permanent, which is over 36 months. ACEMat™ falls into the permanent category.
Additionally, according to the application standards EN 13249 – 13257, EN 13265, and EN
15381, the typical RSL of ACEMat™ is approximately 25 years.
USED RSL (YR) IN THIS LCA CALCULATION:
25
2.4 TECHNICAL DATA
See above (2.1).
2.5 SUBSTANCES OF VERY HIGH CONCERN
The product contains less than 0.1% of substances included in the “Candidate list of
substances of very high concern for authorisation” (SVHC).
2.6 DESCRIPTION PRODUCTION PROCESS
2.2 APPLICATION (INTENDED USE OF THE PRODUCT) The primary material for ACEMat™, PP monofilament, is produced by thoroughly mixing
and stirring various plastic pellets, followed by extrusion and stretching processes. After
ACEMat™, woven into mesh structures with rectangular pyramid patterns, has shown the PP monofilament undergoes the arranging process, it is ready to be fed into the
effectiveness in erosion control and channel protection. This TRM is especially useful in civil production line for weaving ACEMat™. Weaving is a method of fabric production where
engineering for stabilizing slopes. Rain impact can dislodge topsoil, exposing roots and two distinct sets of yarn interlace at right angles, forming a longitudinal warp direction
ACEMat™ | ReTHiNK-58056 4 / 24
Environmental Product Declaration
2 Product
(machine direction) and a transversal weft direction (cross-machine direction). Through
careful textile design, ACEMat™ displays a rectangular arrangement on its surface. After - Placement of ACEMat™
the fabric undergoes heat shrinking, the yarn forms a three-dimensional rectangular
-Execution of anchorage process
pyramid-like structure. Upon passing visual inspection, the fabric is cut to the required
lengths, rolled onto paper tubes for packaging, and then stored in the warehouse.
-Implementation of hydroseeding process
2.7 CONSTRUCTION DESCRIPTION
The construction process for the turf reinforcement mat, ACEMat™, can be categorized
into the following stages:
-Preparation of the site
ACEMat™ | ReTHiNK-58056 5 / 24
Environmental Product Declaration
3 Calculation rules
3.1 DECLARED UNIT Module B2 = Maintenance Module C4 = Disposal
Module D = Benefits and loads beyond the
One square meter ACEMat™ Module B3 = Repair
product system boundaries
m² of ACEMat™. The following products are covered in this EPD: ACEMat™ R, ACEMat™
Module B4 = Replacement
RIII, ACEMat™ R TA, ACEMat™ RIII TA.
reference_unit: square meter (m2)
3.4 REPRESENTATIVENESS
3.2 CONVERSION FACTORS
The input data are representative for ACEMat™, a product of Gold-Joint Industry. The data
are representative for Asia.
Description Value Unit
reference_unit 1 m2
3.5 CUT-OFF CRITERIA
weight_per_reference_unit 1.231 kg
Product Stage (A1-A3)
Conversion factor to 1 kg 0.812414 m2
All input flows (e.g. raw materials, transportation, energy use, packaging, etc.) and output
3.3 SCOPE OF DECLARATION AND SYSTEM BOUNDARIES flows (e.g. production waste) are considered in this LCA. The total neglected input flows do
therefore not exceed the limit of 5% of energy use and mass.
This is a Cradle to gate with options, modules C1-C4 and module D LCA. The life cycle
stages included are as shown below: Construction process stage (A4-A5)
(X = module included, ND = module not declared)
All input flows (e.g. transportation to the construction site, additional raw material use for
A1 A2 A3 A4 A5 B1 B2 B3 B4 B5 B6 B7 C1 C2 C3 C4 D
construction, installation energy (use)of energy use for assembly , etc.) and output flows
X X X X X ND ND ND ND ND ND ND X X X X X (e.g. construction waste, packaging waste, etc.) are considered in this LCA. The total
neglected input flows do therefore not exceed the limit of 5% of energy use and mass.
The modules of the EN15804 contain the following:
End of life stage (C1-C4)
Module A1 = Raw material supply Module B5 = Refurbishment
Module A2 = Transport Module B6 = Operational energy use All input flows (e.g. energy use for demolition or disassembly, transport to waste
processing, etc.) and output flows (e.g. end-of-life waste processing of the product, etc.) are
Module A3 = Manufacturing Module B7 = Operational water use
considered in this LCA. The total neglected input flows do therefore not exceed the limit of
Module A4 = Transport Module C1 = De-construction / Demolition 5% of energy use and mass.
Module A5 = Construction -
Module C2 = Transport
Installation process Benefits and Loads beyond the system boundary (Module D)
Module B1 = Use Module C3 = Waste Processing
ACEMat™ | ReTHiNK-58056 6 / 24
Environmental Product Declaration
3 Calculation rules
All benefits and loads beyond the system boundary resulting from reusable products, [number fixed part]+([specific mass]*[number scalable part])
recyclable materials and/or useful energy carriers leaving the product system are
considered in this LCA. The input cardboard tube did not have a linear dependence on the specific mass, so the
higher quantity of product available was always taken into account to make the scaling as
conservative as possible.
3.6 ALLOCATION
The input cardboard tube was not having a linear dependance on the specific mass, thus
Allocation is based on physical characteristics, on mass. The production data was the higher amount of the product available was always considered for the scaling to be as
calculated according to the annual quantity by mass. The raw materials and energy were conservative as possible.
calculated according to this allocation key.
For C1 the method and amount of the generic data set 'Polyester weefsel' from chapter
22.46 Grondwapening en grondscheiding of the DuboCalc programme (database version
3.7 DATA COLLECTION & REFERENCE TIME PERIOD NMD 1.8 - 5.01.14052018) was used. In this generic data set, 0.0013h work per m² of
geotextile was assumed.
All process-specific data was collected for the operating year 2021.
3.9 DATA QUALITY
3.8 ESTIMATES AND ASSUMPTIONS
All process-specific data was collected for the 2021 operating year and is therefore up-to-
date. The data is based on the annual average. In order to ensure comparability of the
Almost all the datasets selected for the LCA refer to the RoW as the geographical
results, only consistent background data of the Ecoinvent database V3.6 was used in the
reference, as there were no specific environmental profiles available.
LCA (e.g., records on energy, transportation, and supplies), which refers to reference year
Gold-Joint delivers its product to different countries, so the calculation of transport to 2019. The database is regularly reviewed and thus complies with the requirements of EN
construction site (A4) was done by taking the average distance, weighted by the 15804 (background data not older than 10 years). All consistent datasets contained in the
proportion of product shipped to each country. For module A4, a data set for a non- Ecoinvent database are documented and can be viewed in the online Ecoinvent
specific truck and a transoceanic ship was used. documentation. The primary data were provided by Gold-Joint. The life cycle was modelled
with the R<THiNK EPD App.
A scaling method was used to calculate the LCA results for the different ACEMat™
products. The scaling was done on the basis of mass per square meter. As a result of
scaling there are results for both the fixed and the scalable part of the scaling function. 3.10 GUARANTEES OF ORIGIN
The fixed part means that this number is the same for each product in the product group
and the scalable part is the part that depends on the mass per unit area of the product. In In this EPD, the local based approach was considered for the LCA, therefore no guaranties
order to calculate the correct number of each environmental impact category for each of of origin (GO) are needed.
the products in the product group, the following calculation should be done:
ACEMat™ | ReTHiNK-58056 7 / 24
Environmental Product Declaration
3 Calculation rules
3.12 SCALING
Parameter Value
Scaling type Linear
Description dimension Specific mass
Dimension 0.000
Scalable dimension 1.000
Unit dimension kg/m²
ACEMat™ | ReTHiNK-58056 8 / 24
Environmental Product Declaration
4 Scenarios and additional technical information
4.1 TRANSPORT TO CONSTRUCTION SITE (A4)
For the transport from production place to assembly/user, the following scenario is
assumed for module A4 of this EPD.
Value and unit
Vehicle type used for transport Transoceanic ship / Lorry unspecified
Fuel type and consumption of vehicle
Distance 5591 km
Capacity utilisation (including empty returns)
Bulk density of transported products
Volume capacity utilisation factor
4.2 ASSEMBLY (A5)
The following information describes the scenarios for flows entering the system and flows
leaving the system at module A5.
FLOWS ENTERING THE SYSTEM
For flows entering the system at A5 the following scenario is assumed for module A5.
Value Unit
Materials used for installation/assembly
Glass fibre reinforced plastic, polyamide, injection moulded {RoW}| production | Cut-off, U 0.11235 kg
FLOWS LEAVING THE SYSTEM
The following output flows leaving the system at module A5 are assumed.
Description Value Unit
Output materials as result of loss during construction 5 %
Output materials as result of waste processing of materials used for installation/assembly at the building site 0.112 kg
Output materials as result of waste processing of used packaging 0.054 kg
4.3 DE-CONSTRUCTION, DEMOLITION (C1)
The following information describes the scenario for demolition at end of life.
ACEMat™ | ReTHiNK-58056 9 / 24
Environmental Product Declaration
4 Scenarios and additional technical information
Description Amount Unit
Hydraulic excavator (average) [NMD] 0.001 hr
4.4 TRANSPORT END-OF-LIFE (C2)
The following distances and transport conveyance are assumed for transportation during
end of life for the different types of waste processing.
Waste Scenario Transport conveyance Not removed (stays in Landfill Incineration Recycling Re-use
work) [km] [km] [km] [km] [km]
PE/PP soil reinforcement (geotextile and Lorry (Truck), unspecified (default) | market
0 100 150 50 0
geogrid 54) group for (GLO)
finishes (adhered to wood, plastic, metal) Lorry (Truck), unspecified (default) | market
0 100 150 50 0
(NMD ID 2) group for (GLO)
The transport conveyance(s) used in the scenario(s) for transport during end of life has the
following characteristics.
Value and unit
Vehicle type used for transport Lorry (Truck), unspecified (default) | market group for (GLO)
Fuel type and consumption of vehicle not available
Capacity utilisation (including empty returns) 50 % (loaded up and return empty)
Bulk density of transported products inapplicable
Volume capacity utilisation factor 1
4.5 END OF LIFE (C3, C4)
The scenario(s) assumed for end of life of the product are given in the following tables.
First the assumed percentages per type of waste processing are displayed, followed by the
assumed amounts.
Waste Scenario Region Not removed (stays in work) [%] Landfill [%] Incineration [%] Recycling [%] Re-use [%]
PE/PP soil reinforcement (geotextile and geogrid 54) NL 25 0 70 5 0
ACEMat™ | ReTHiNK-58056 10 / 24
Environmental Product Declaration
4 Scenarios and additional technical information
Waste Scenario Region Not removed (stays in work) [%] Landfill [%] Incineration [%] Recycling [%] Re-use [%]
finishes (adhered to wood, plastic, metal) (NMD ID 2) NL 0 0 100 0 0
Waste Scenario Not removed (stays in work) [kg] Landfill [kg] Incineration [kg] Recycling [kg] Re-use [kg]
PE/PP soil reinforcement (geotextile and geogrid 54) 0.322 0.000 0.902 0.064 0.000
finishes (adhered to wood, plastic, metal) (NMD ID 2) 0.000 0.000 0.014 0.000 0.000
Total 0.322 0.000 0.916 0.064 0.000
4.6 BENEFITS AND LOADS BEYOND THE SYSTEM BOUNDARY (D)
The presented Benefits and loads beyond the system boundary in this EPD are based on
the following calculated Net output flows in kilograms and Energy recovery displayed in
MJ Lower Heating Value.
Waste Scenario Net output flow [kg] Energy recovery [MJ]
PE/PP soil reinforcement (geotextile and geogrid 54) 0.061 33.846
finishes (adhered to wood, plastic, metal) (NMD ID 2) 0.000 0.000
Total 0.061 33.846
ACEMat™ | ReTHiNK-58056 11 / 24
Environmental Product Declaration
5 Results
For the impact assessment, the characterization factors of the LCIA method EN 15804 +A2
Method v1.0 are used. Long-term emissions (>100 years) are not considered in the impact
assessment. The results of the impact assessment are only relative statements that do not
make any statements about end-points of the impact categories, exceedance of threshold
values, safety margins or risks. The following tables show the results of the indicators of the
impact assessment, of the use of resources as well as of waste and other output flows.
ACEMat™ | ReTHiNK-58056 12 / 24
Environmental Product Declaration
5 Results
5.1 ENVIRONMENTAL IMPACT INDICATORS PER SQUARE METER (FIXED PART)
CORE ENVIRONMENTAL IMPACT INDICATORS EN15804+A2
Abbreviation Unit A1 A2 A3 A4 A5 C1 C2 C3 C4 D
AP mol H+ eqv. -6.87E-4 -9.90E-6 9.30E-6 -1.17E-4 4.54E-3 7.12E-4 -6.11E-6 -6.07E-5 -1.65E-6 9.73E-5
GWP-total kg CO2 eqv. -1.72E-1 -1.71E-3 -5.61E-3 -1.00E-2 1.33E+0 6.81E-2 -1.05E-3 -1.36E-1 -2.65E-3 9.47E-2
GWP-b kg CO2 eqv. -1.90E-4 -7.88E-7 -2.22E-4 -6.19E-6 1.81E-2 1.89E-5 -4.86E-7 -1.95E-5 -2.04E-6 6.20E-5
GWP-f kg CO2 eqv. -1.71E-1 -1.71E-3 -5.45E-3 -9.99E-3 1.31E+0 6.81E-2 -1.05E-3 -1.36E-1 -2.65E-3 9.47E-2
GWP-luluc kg CO2 eqv. -5.21E-5 -6.26E-7 6.42E-5 -4.14E-6 2.26E-4 5.37E-6 -3.86E-7 -1.09E-5 -9.37E-8 -2.70E-7
EP-m kg N eqv. -1.17E-4 -3.49E-6 9.07E-6 -2.91E-5 1.41E-3 3.14E-4 -2.15E-6 -1.66E-5 -1.00E-6 2.57E-5
EP-fw kg P eqv. -3.68E-6 -1.72E-8 2.76E-7 -1.18E-7 1.17E-5 2.48E-7 -1.06E-8 -4.05E-7 -3.40E-9 1.90E-7
EP-T mol N eqv. -1.30E-3 -3.85E-5 7.87E-5 -3.25E-4 7.94E-3 3.45E-3 -2.37E-5 -1.85E-4 -6.08E-6 2.82E-4
kg CFC 11
ODP -3.39E-9 -3.77E-10 1.00E-9 -2.13E-9 2.05E-8 1.47E-8 -2.33E-10 -4.11E-9 -5.86E-11 1.15E-8
eqv.
kg NMVOC
POCP -5.40E-4 -1.10E-5 -5.65E-6 -8.88E-5 2.64E-3 9.49E-4 -6.78E-6 -4.97E-5 -2.33E-6 1.01E-4
eqv.
ADP-f MJ -5.38E+0 -2.57E-2 -1.00E-1 -1.48E-1 1.47E+1 9.37E-1 -1.59E-2 -1.05E-1 -4.49E-3 1.72E+0
ADP-mm kg Sb-eqv. -1.57E-6 -4.33E-8 -1.01E-8 -1.75E-7 2.09E-6 1.04E-7 -2.67E-8 -1.72E-7 -2.03E-9 8.66E-8
m3 world
WDP -6.34E-2 -9.21E-5 3.40E-5 -6.48E-4 9.81E-1 1.26E-3 -5.68E-5 -6.84E-3 -1.92E-4 1.24E-2
eqv.
AP=Acidification (AP) | GWP-total=Global warming potential (GWP-total) | GWP-b=Global warming potential - Biogenic (GWP-b) | GWP-f=Global warming potential - Fossil (GWP-f) | GWP-
luluc=Global warming potential - Land use and land use change (GWP-luluc) | EP-m=Eutrophication marine (EP-m) | EP-fw=Eutrophication, freshwater (EP-fw) | EP-T=Eutrophication,
terrestrial (EP-T) | ODP=Ozone depletion (ODP) | POCP=Photochemical ozone formation - human health (POCP) | ADP-f=Resource use, fossils (ADP-f) | ADP-mm=Resource use, minerals and
metals (ADP-mm) | WDP=Water use (WDP)
ACEMat™ | ReTHiNK-58056 13 / 24
Environmental Product Declaration
5 Results
ADDITIONAL ENVIRONMENTAL IMPACT INDICATORS EN15084+A2
Abbreviation Unit A1 A2 A3 A4 A5 C1 C2 C3 C4 D
ETP-fw CTUe -2.02E+0 -2.30E-2 8.82E-1 -1.22E-1 4.40E+0 5.65E-1 -1.42E-2 -1.69E+0 -4.77E-3 1.24E-1
disease
PM -5.62E-9 -1.54E-10 4.47E-10 -7.07E-10 4.94E-8 1.89E-8 -9.48E-11 -4.92E-10 -3.12E-11 4.11E-10
incidence
HTP-c CTUh -3.97E-11 -7.45E-13 -8.75E-12 -3.99E-12 5.18E-10 1.97E-11 -4.60E-13 -2.82E-11 -1.25E-13 7.29E-12
HTP-nc CTUh -1.24E-9 -2.51E-11 1.70E-11 -1.23E-10 4.18E-9 4.85E-10 -1.55E-11 -5.41E-10 -3.11E-12 1.19E-10
IR kBq U235 eqv. -1.74E-3 -1.08E-4 5.34E-5 -6.30E-4 1.13E-2 4.02E-3 -6.66E-5 -4.29E-4 -1.76E-5 6.33E-4
SQP Pt -1.94E-1 -2.23E-2 3.72E-1 -9.41E-2 1.42E+0 1.20E-1 -1.38E-2 -3.86E-2 -1.06E-2 -6.00E-1
ETP-fw=Ecotoxicity, freshwater (ETP-fw) | PM=Particulate Matter (PM) | HTP-c=Human toxicity, cancer (HTP-c) | HTP-nc=Human toxicity, non-cancer (HTP-nc) | IR=Ionising radiation, human
health (IR) | SQP=Land use (SQP)
CLASSIFICATION OF DISCLAIMERS TO THE DECLARATION OF CORE AND ADDITIONAL ENVIRONMENTAL IMPACT INDICATORS
ILCD classification Indicator Disclaimer
Global warming potential (GWP) None
ILCD type / level 1 Depletion potential of the stratospheric ozone layer (ODP) None
Potential incidence of disease due to PM emissions (PM) None
AAcidification potential, Accumulated Exceedance (AP) None
Eutrophication potential, Fraction of nutrients reaching freshwater end compartment
None
(EP-freshwater)
Eutrophication potential, Fraction of nutrients reaching marine end compartment
ILCD type / level 2 None
(EP-marine)
Eutrophication potential, Accumulated Exceedance (EP-terrestrial) None
Formation potential of tropospheric ozone (POCP) None
Potential Human exposure efficiency relative to U235 (IRP) 1
Abiotic depletion potential for non-fossil resources (ADP-minerals&metals) 2
ILCD type / level 3
Abiotic depletion potential for fossil resources (ADP-fossil) 2
Water (user) deprivation potential, deprivation-weighted water consumption (WDP) 2
Potential Comparative Toxic Unit for ecosystems (ETP-fw) 2
ACEMat™ | ReTHiNK-58056 14 / 24
Environmental Product Declaration
5 Results
ILCD classification Indicator Disclaimer
Potential Comparative Toxic Unit for humans (HTP-c) 2
Potential Comparative Toxic Unit for humans (HTP-nc) 2
Potential Soil quality index (SQP) 2
Disclaimer 1 – This impact category deals mainly with the eventual impact of low dose ionizing radiation on human health of the nuclear fuel cycle. It does not consider effects due to possible
nuclear accidents, occupational exposure nor due to radioactive waste disposal in underground facilities. Potential ionizing radiation from the soil, from radon and from some construction
materials is also not measured by this indicator.
Disclaimer 2 – The results of this environmental impact indicator shall be used with care as the uncertainties on these results are high or as there is limited experienced with the indicator.
5.2 ENVIRONMENTAL IMPACT INDICATORS PER SQUARE METER (SCALABLE PART)
CORE ENVIRONMENTAL IMPACT INDICATORS EN15804+A2
Abbreviation Unit A1 A2 A3 A4 A5 C1 C2 C3 C4 D
AP mol H+ eqv. 1.24E-2 3.86E-5 9.01E-3 2.62E-3 1.28E-3 0.00E+0 1.10E-4 1.09E-3 2.98E-5 -1.83E-3
GWP-total kg CO2 eqv. 3.10E+0 6.66E-3 2.22E+0 2.23E-1 5.16E-1 0.00E+0 1.90E-2 2.45E+0 4.78E-2 -1.78E+0
GWP-b kg CO2 eqv. 3.42E-3 3.07E-6 -8.14E-3 1.38E-4 -2.03E-4 0.00E+0 8.77E-6 3.52E-4 3.68E-5 -1.14E-3
GWP-f kg CO2 eqv. 3.09E+0 6.65E-3 2.23E+0 2.23E-1 5.16E-1 0.00E+0 1.90E-2 2.45E+0 4.78E-2 -1.78E+0
GWP-luluc kg CO2 eqv. 9.36E-4 2.44E-6 1.90E-4 9.23E-5 7.20E-5 0.00E+0 6.96E-6 1.97E-4 1.69E-6 -8.82E-5
EP-m kg N eqv. 2.11E-3 1.36E-5 1.22E-3 6.50E-4 2.24E-4 0.00E+0 3.88E-5 3.00E-4 1.81E-5 -4.87E-4
EP-fw kg P eqv. 6.63E-5 6.71E-8 6.47E-5 2.63E-6 7.09E-6 0.00E+0 1.92E-7 7.30E-6 6.13E-8 -4.07E-6
EP-T mol N eqv. 2.35E-2 1.50E-4 1.36E-2 7.24E-3 2.50E-3 0.00E+0 4.28E-4 3.34E-3 1.10E-4 -5.36E-3
kg CFC 11
ODP 6.05E-8 1.47E-9 8.84E-8 4.75E-8 1.48E-8 0.00E+0 4.19E-9 7.41E-8 1.06E-9 -2.17E-7
eqv.
kg NMVOC
POCP 9.72E-3 4.28E-5 4.43E-3 1.98E-3 8.84E-4 0.00E+0 1.22E-4 8.97E-4 4.20E-5 -1.92E-3
eqv.
AP=Acidification (AP) | GWP-total=Global warming potential (GWP-total) | GWP-b=Global warming potential - Biogenic (GWP-b) | GWP-f=Global warming potential - Fossil (GWP-f) | GWP-
luluc=Global warming potential - Land use and land use change (GWP-luluc) | EP-m=Eutrophication marine (EP-m) | EP-fw=Eutrophication, freshwater (EP-fw) | EP-T=Eutrophication,
terrestrial (EP-T) | ODP=Ozone depletion (ODP) | POCP=Photochemical ozone formation - human health (POCP) | ADP-f=Resource use, fossils (ADP-f) | ADP-mm=Resource use, minerals and
metals (ADP-mm) | WDP=Water use (WDP)
ACEMat™ | ReTHiNK-58056 15 / 24
Environmental Product Declaration
5 Results
Abbreviation Unit A1 A2 A3 A4 A5 C1 C2 C3 C4 D
ADP-f MJ 9.71E+1 1.00E-1 3.28E+1 3.30E+0 6.89E+0 0.00E+0 2.86E-1 1.89E+0 8.09E-2 -3.23E+1
ADP-mm kg Sb-eqv. 2.83E-5 1.69E-7 5.09E-6 3.90E-6 2.09E-6 0.00E+0 4.81E-7 3.11E-6 3.66E-8 -1.65E-6
m3 world
WDP 1.14E+0 3.59E-4 3.38E-1 1.45E-2 8.11E-2 0.00E+0 1.02E-3 1.23E-1 3.46E-3 -2.28E-1
eqv.
AP=Acidification (AP) | GWP-total=Global warming potential (GWP-total) | GWP-b=Global warming potential - Biogenic (GWP-b) | GWP-f=Global warming potential - Fossil (GWP-f) | GWP-
luluc=Global warming potential - Land use and land use change (GWP-luluc) | EP-m=Eutrophication marine (EP-m) | EP-fw=Eutrophication, freshwater (EP-fw) | EP-T=Eutrophication,
terrestrial (EP-T) | ODP=Ozone depletion (ODP) | POCP=Photochemical ozone formation - human health (POCP) | ADP-f=Resource use, fossils (ADP-f) | ADP-mm=Resource use, minerals and
metals (ADP-mm) | WDP=Water use (WDP)
ADDITIONAL ENVIRONMENTAL IMPACT INDICATORS EN15084+A2
Abbreviation Unit A1 A2 A3 A4 A5 C1 C2 C3 C4 D
ETP-fw CTUe 3.64E+1 8.95E-2 2.31E+1 2.72E+0 4.70E+0 0.00E+0 2.55E-1 3.04E+1 8.60E-2 -2.35E+0
disease
PM 1.01E-7 5.99E-10 2.78E-8 1.58E-8 7.99E-9 0.00E+0 1.71E-9 8.87E-9 5.62E-10 -7.84E-9
incidence
HTP-c CTUh 7.13E-10 2.90E-12 5.89E-10 8.91E-11 2.33E-10 0.00E+0 8.28E-12 5.06E-10 2.26E-12 -1.39E-10
HTP-nc CTUh 2.24E-8 9.79E-11 1.59E-8 2.75E-9 3.00E-9 0.00E+0 2.79E-10 9.75E-9 5.60E-11 -2.30E-9
IR kBq U235 eqv. 3.12E-2 4.20E-4 8.02E-2 1.41E-2 6.86E-3 0.00E+0 1.20E-3 7.73E-3 3.17E-4 -1.20E-2
SQP Pt 3.49E+0 8.70E-2 2.89E+0 2.10E+0 5.01E-1 0.00E+0 2.48E-1 6.96E-1 1.91E-1 -5.52E-1
ETP-fw=Ecotoxicity, freshwater (ETP-fw) | PM=Particulate Matter (PM) | HTP-c=Human toxicity, cancer (HTP-c) | HTP-nc=Human toxicity, non-cancer (HTP-nc) | IR=Ionising radiation, human
health (IR) | SQP=Land use (SQP)
CLASSIFICATION OF DISCLAIMERS TO THE DECLARATION OF CORE AND ADDITIONAL ENVIRONMENTAL IMPACT INDICATORS
ILCD classification Indicator Disclaimer
Global warming potential (GWP) None
ILCD type / level 1 Depletion potential of the stratospheric ozone layer (ODP) None
Potential incidence of disease due to PM emissions (PM) None
AAcidification potential, Accumulated Exceedance (AP) None
ILCD type / level 2
None
ACEMat™ | ReTHiNK-58056 16 / 24
Environmental Product Declaration
5 Results
ILCD classification Indicator Disclaimer
Eutrophication potential, Fraction of nutrients reaching freshwater end compartment
(EP-freshwater)
Eutrophication potential, Fraction of nutrients reaching marine end compartment
None
(EP-marine)
Eutrophication potential, Accumulated Exceedance (EP-terrestrial) None
Formation potential of tropospheric ozone (POCP) None
Potential Human exposure efficiency relative to U235 (IRP) 1
Abiotic depletion potential for non-fossil resources (ADP-minerals&metals) 2
Abiotic depletion potential for fossil resources (ADP-fossil) 2
Water (user) deprivation potential, deprivation-weighted water consumption (WDP) 2
ILCD type / level 3 Potential Comparative Toxic Unit for ecosystems (ETP-fw) 2
Potential Comparative Toxic Unit for humans (HTP-c) 2
Potential Comparative Toxic Unit for humans (HTP-nc) 2
Potential Soil quality index (SQP) 2
Disclaimer 1 – This impact category deals mainly with the eventual impact of low dose ionizing radiation on human health of the nuclear fuel cycle. It does not consider effects due to possible
nuclear accidents, occupational exposure nor due to radioactive waste disposal in underground facilities. Potential ionizing radiation from the soil, from radon and from some construction
materials is also not measured by this indicator.
Disclaimer 2 – The results of this environmental impact indicator shall be used with care as the uncertainties on these results are high or as there is limited experienced with the indicator.
ACEMat™ | ReTHiNK-58056 17 / 24
Environmental Product Declaration
5 Results
5.3 ENVIRONMENTAL IMPACT INDICATORS PER SQUARE METER (FIXED PART)
PARAMETERS DESCRIBING RESOURCE USE
Abbreviation Unit A1 A2 A3 A4 A5 C1 C2 C3 C4 D
PERE MJ -6.09E-2 -3.22E-4 6.99E-2 -2.21E-3 4.55E-1 5.07E-3 -1.99E-4 -1.06E-2 -7.94E-5 -1.01E-1
PERM MJ 0.00E+0 0.00E+0 0.00E+0 0.00E+0 0.00E+0 0.00E+0 0.00E+0 0.00E+0 0.00E+0 0.00E+0
PERT MJ -6.09E-2 -3.22E-4 6.99E-2 -2.21E-3 4.55E-1 5.07E-3 -1.99E-4 -1.06E-2 -7.94E-5 -1.01E-1
PENRE MJ -2.77E+0 -2.73E-2 -1.22E-1 -1.57E-1 1.60E+1 9.95E-1 -1.69E-2 -1.11E-1 -4.77E-3 1.74E+0
PENRM MJ -3.01E+0 0.00E+0 1.90E-2 0.00E+0 -1.49E-1 0.00E+0 0.00E+0 0.00E+0 0.00E+0 1.59E-1
PENRT MJ -5.78E+0 -2.73E-2 -1.03E-1 -1.57E-1 1.58E+1 9.95E-1 -1.69E-2 -1.11E-1 -4.77E-3 1.90E+0
SM Kg 0.00E+0 0.00E+0 0.00E+0 0.00E+0 0.00E+0 0.00E+0 0.00E+0 0.00E+0 0.00E+0 0.00E+0
RSF MJ 0.00E+0 0.00E+0 0.00E+0 0.00E+0 0.00E+0 0.00E+0 0.00E+0 0.00E+0 0.00E+0 0.00E+0
NRSF MJ 0.00E+0 0.00E+0 0.00E+0 0.00E+0 0.00E+0 0.00E+0 0.00E+0 0.00E+0 0.00E+0 0.00E+0
FW M3 -1.56E-3 -3.14E-6 1.74E-5 -2.13E-5 2.34E-2 4.83E-5 -1.94E-6 -2.01E-4 -4.68E-6 1.74E-4
PERE=renewable primary energy ex. raw materials | PERM=renewable primary energy used as raw materials | PERT=renewable primary energy total | PENRE=non-renewable primary energy
ex. raw materials | PENRM=non-renewable primary energy used as raw materials | PENRT=non-renewable primary energy total | SM=use of secondary material | RSF=use of renewable
secondary fuels | NRSF=use of non-renewable secondary fuels | FW=use of net fresh water
OTHER ENVIRONMENTAL INFORMATION DESCRIBING WASTE CATEGORIES
Abbreviation Unit A1 A2 A3 A4 A5 C1 C2 C3 C4 D
HWD Kg -5.93E-7 -6.52E-8 1.64E-7 -2.93E-7 6.79E-6 2.55E-6 -4.03E-8 -2.02E-7 -6.82E-9 1.87E-6
NHWD Kg -8.60E-3 -1.63E-3 1.13E-3 -6.42E-3 8.62E-2 1.11E-3 -1.01E-3 -2.61E-3 -1.79E-2 7.24E-4
RWD Kg -1.62E-6 -1.69E-7 4.57E-8 -9.68E-7 1.12E-5 6.51E-6 -1.04E-7 -3.77E-7 -2.67E-8 8.35E-7
HWD=hazardous waste disposed | NHWD=non hazardous waste disposed | RWD=radioactive waste disposed
ACEMat™ | ReTHiNK-58056 18 / 24
Environmental Product Declaration
5 Results
ENVIRONMENTAL INFORMATION DESCRIBING OUTPUT FLOWS
Abbreviation Unit A1 A2 A3 A4 A5 C1 C2 C3 C4 D
CRU Kg 0.00E+0 0.00E+0 0.00E+0 0.00E+0 0.00E+0 0.00E+0 0.00E+0 0.00E+0 0.00E+0 0.00E+0
MFR Kg 0.00E+0 0.00E+0 0.00E+0 0.00E+0 9.27E-3 0.00E+0 0.00E+0 -3.58E-3 0.00E+0 0.00E+0
MER Kg 0.00E+0 0.00E+0 0.00E+0 0.00E+0 0.00E+0 0.00E+0 0.00E+0 0.00E+0 0.00E+0 0.00E+0
EET MJ 0.00E+0 0.00E+0 -4.40E-2 0.00E+0 0.00E+0 0.00E+0 0.00E+0 0.00E+0 0.00E+0 -6.50E-1
EEE MJ 0.00E+0 0.00E+0 -2.56E-2 0.00E+0 0.00E+0 0.00E+0 0.00E+0 0.00E+0 0.00E+0 -3.77E-1
CRU=Components for re-use | MFR=Materials for recycling | MER=Materials for energy recovery | EET=Exported Energy Thermic | EEE=Exported Energy Electric
5.4 ENVIRONMENTAL IMPACT INDICATORS PER SQUARE METER (SCALABLE PART)
PARAMETERS DESCRIBING RESOURCE USE
Abbreviation Unit A1 A2 A3 A4 A5 C1 C2 C3 C4 D
PERE MJ 1.09E+0 1.26E-3 1.20E+0 4.92E-2 1.28E-1 0.00E+0 3.58E-3 1.91E-1 1.43E-3 -1.39E-1
PERM MJ 0.00E+0 0.00E+0 0.00E+0 0.00E+0 0.00E+0 0.00E+0 0.00E+0 0.00E+0 0.00E+0 0.00E+0
PERT MJ 1.09E+0 1.26E-3 1.20E+0 4.92E-2 1.28E-1 0.00E+0 3.58E-3 1.91E-1 1.43E-3 -1.39E-1
PENRE MJ 4.99E+1 1.07E-1 3.05E+1 3.50E+0 4.45E+0 0.00E+0 3.04E-1 2.01E+0 8.60E-2 -3.28E+1
PENRM MJ 5.42E+1 0.00E+0 4.31E+0 0.00E+0 2.93E+0 0.00E+0 0.00E+0 0.00E+0 0.00E+0 -2.87E+0
PENRT MJ 1.04E+2 1.07E-1 3.48E+1 3.50E+0 7.37E+0 0.00E+0 3.04E-1 2.01E+0 8.60E-2 -3.56E+1
SM Kg 0.00E+0 0.00E+0 0.00E+0 0.00E+0 0.00E+0 0.00E+0 0.00E+0 0.00E+0 0.00E+0 0.00E+0
RSF MJ 0.00E+0 0.00E+0 0.00E+0 0.00E+0 0.00E+0 0.00E+0 0.00E+0 0.00E+0 0.00E+0 0.00E+0
NRSF MJ 0.00E+0 0.00E+0 0.00E+0 0.00E+0 0.00E+0 0.00E+0 0.00E+0 0.00E+0 0.00E+0 0.00E+0
FW M3 2.81E-2 1.22E-5 9.41E-3 4.74E-4 2.10E-3 0.00E+0 3.49E-5 3.63E-3 8.44E-5 -3.23E-3
PERE=renewable primary energy ex. raw materials | PERM=renewable primary energy used as raw materials | PERT=renewable primary energy total | PENRE=non-renewable primary energy
ex. raw materials | PENRM=non-renewable primary energy used as raw materials | PENRT=non-renewable primary energy total | SM=use of secondary material | RSF=use of renewable
secondary fuels | NRSF=use of non-renewable secondary fuels | FW=use of net fresh water
ACEMat™ | ReTHiNK-58056 19 / 24
Environmental Product Declaration
5 Results
OTHER ENVIRONMENTAL INFORMATION DESCRIBING WASTE CATEGORIES
Abbreviation Unit A1 A2 A3 A4 A5 C1 C2 C3 C4 D
HWD Kg 1.06E-5 2.54E-7 1.07E-5 6.54E-6 1.92E-6 0.00E+0 7.26E-7 3.64E-6 1.23E-7 -3.54E-5
NHWD Kg 1.55E-1 6.37E-3 1.17E-1 1.43E-1 4.32E-2 0.00E+0 1.82E-2 4.71E-2 3.23E-1 -1.53E-2
RWD Kg 2.89E-5 6.59E-7 7.11E-5 2.16E-5 6.73E-6 0.00E+0 1.88E-6 6.79E-6 4.81E-7 -1.60E-5
HWD=hazardous waste disposed | NHWD=non hazardous waste disposed | RWD=radioactive waste disposed
ENVIRONMENTAL INFORMATION DESCRIBING OUTPUT FLOWS
Abbreviation Unit A1 A2 A3 A4 A5 C1 C2 C3 C4 D
CRU Kg 0.00E+0 0.00E+0 0.00E+0 0.00E+0 0.00E+0 0.00E+0 0.00E+0 0.00E+0 0.00E+0 0.00E+0
MFR Kg 0.00E+0 0.00E+0 0.00E+0 0.00E+0 3.22E-3 0.00E+0 0.00E+0 6.45E-2 0.00E+0 0.00E+0
MER Kg 0.00E+0 0.00E+0 0.00E+0 0.00E+0 0.00E+0 0.00E+0 0.00E+0 0.00E+0 0.00E+0 0.00E+0
EET MJ 0.00E+0 0.00E+0 7.93E-1 0.00E+0 0.00E+0 0.00E+0 0.00E+0 0.00E+0 0.00E+0 1.22E+1
EEE MJ 0.00E+0 0.00E+0 4.61E-1 0.00E+0 0.00E+0 0.00E+0 0.00E+0 0.00E+0 0.00E+0 7.10E+0
CRU=Components for re-use | MFR=Materials for recycling | MER=Materials for energy recovery | EET=Exported Energy Thermic | EEE=Exported Energy Electric
ACEMat™ | ReTHiNK-58056 20 / 24
Environmental Product Declaration
5 Results
5.5 INFORMATION ON BIOGENIC CARBON CONTENT PER SQUARE METER
BIOGENIC CARBON CONTENT
The following Information describes the biogenic carbon content in (the main parts of) the
product at the factory gate per square meter:
Biogenic carbon content Amount Unit
Biogenic carbon content in the product 0 kg C
Biogenic carbon content in accompanying packaging 0 kg C
ACEMat™ | ReTHiNK-58056 21 / 24
Environmental Product Declaration
6 Interpretation of results
As shown in the figure below, the production process (A3) dominates in most
environmental core indicators, followed by installation into the building (A5) and
production process (A3). The highest influence on the Global Warming Potential have raw
material supply (A1), production process (A3) and waste processing (C3). Transports (A2, C2)
have rather a minor impact within all core indicators.
ACEMat™ | ReTHiNK-58056 22 / 24
Environmental Product Declaration
7 References
ISO 14040
ISO 14040:2006-10, Environmental management - Life cycle assessment - Principles and
framework; EN ISO 14040:2006
ISO 14044
ISO 14044:2006-10, Environmental management - Life cycle assessment - Requirements
and guidelines; EN ISO 14040:2006
ISO 14025
ISO 14025:2011-10: Environmental labels and declarations — Type III environmental
declarations — Principles and procedures
EN 15804+A2
EN 15804+A2: 2019: Sustainability of construction works — Environmental Product
Declarations — Core rules for the product category of construction products
PCR A: General Program Category Rules for Construction Products from the EPD program
Kiwa-Ecobility Experts, 2022-02-14
PCR B: Product Category Rules (PCR) from the Kiwa-Ecobility Experts (Kiwa-EE) – Specific
Product Category Rules: Geosynthetic products, 2023-07-21
ACEMat™ | ReTHiNK-58056 23 / 24
Environmental Product Declaration
8 Contact information
Publisher Operator Owner of declaration
Kiwa-Ecobility Experts Kiwa-Ecobility Experts Gold-Joint Industry Co., Ltd.
Voltastraße 5 Voltastraße 5 No.33, Jing 3 Rd. Wuqi Dist.
13355 Berlin, DE 13355 Berlin, DE 43541 Taichung City, Taiwan (R.O.C.), TW
E-mail: E-mail: E-mail:
DE.Ecobility.Experts@kiwa.com DE.Ecobility.Experts@kiwa.com marketing@geoace.com
Website: Website: Website:
https://www.kiwa.com/de/en/themes/ecobility-experts/ecobility-https://www.kiwa.com/de/en/themes/ecobility-experts/ecobility-www.geoace.com
experts-epd-program/ experts-epd-program/
Kiwa-Ecobility Experts is
established member of the
ACEMat™ | ReTHiNK-58056 24 / 24
