Environmental Product
Declaration
as per ISO 14025 and EN 15804+A2
Owner of the declaration: Tensar International Limited
Publisher: Kiwa-Ecobility Experts
Programme operator: Kiwa-Ecobility Experts
Registration number: EPD-TENSAR-161-EN (Rev.1_20.05.2022)
Issue date: 14.12.2021
Valid to: 14.12.2026
Tensar® RE510 geogrid
High performance geogrid used for soil reinforcement solutions
1. General information
Tensar International Limited Tensar® RE510
Programme operator Owner of the declaration
Kiwa-Ecobility Experts Tensar International Limited
Voltastr. 5 Units 2-4 Cunningham Court
13355 Berlin Shadsworth Business Park
Germany Blackburn, United Kingdom
Registration number Declared product / declared unit
EPD-TENSAR-161-EN (Rev.1_20.05.2022) 1 m2 geogrid
This declaration is based on the Product Scope
Category Rules Tensar® RE510 geogrid is a product of the
PCR B – Geosynthetic products 2022-02-08 product series RE500. It is produced and dis-
(draft) tributed by Tensar International Limited, lo-
Issue date cated in Blackburn (United Kingdom). The EPD
14.12.2021 refers to the specific product.
EPD type: Cradle to gate with options, and
Valid to with modules C1-C4 and module D.
14.12.2026 Kiwa-Ecobility Experts shall not be liable with
respect to manufacturer information, life cy-
cle assessment data and evidence.
Verification
The European standard
EN15804:2012+A2:2019 serves as the core
PCR.
Independent verification of the declaration
and data according to ISO 14025:2006
☐internal ☒external
Frank Huppertz
(Head of Kiwa-Ecobility Experts)
Prof. Dr. Frank Heimbecher Anne Kees Jeeninga - Advieslab V.o.f.
(Chairman of the independent expert committee – (Third party verifier)
Kiwa-Ecobility Experts)
Page | 2 Tensar International Limited – Tensar® RE510
2. Product
2.1 Product description
Tensar® RE500 products are uniaxial geogrids made from select grades of high-density polyethylene
(HDPE) resins. The polymer structure is highly oriented to resist elongation (creep) under sustained
tensile load. The products are resistant to installation damage and chemical and biological long-term
degradation.
2.2 Application
Tensar® RE500 geogrids are used for the reinforcement of soils in the construction of structures such
as retaining walls, bridge abutments, steep slopes, slip repairs, cellular foundation, or basal mattresses.
2.3 Technical data
Name Value/Tolerance Unit
Weight of product /TR 041 B.1/ 290 g/m²
Tensile Strength (EN ISO 10319) MD – 46.2/-4.0 kN/m
Elongation at Maximum Load (EN ISO 12236) MD – 11.0/ ±3.0 %
Static Puncture (CBR test) (EN ISO 12236) NPD kN/m
Dynamic Perforation Resistance (cone drop test) (EN
NPD mm
ISO 13433)
Tensile creep (EN ISO 13431)
20.7 kN/m
Long term creep rupture strength at a design life of 120 years and 10ºC
in soil temperature
Damage during Installation
Retained Strength >90/-0 %
(EN ISO 10722-1)
Less than required by na-
Dangerous substances (National Regulations in force
tional regulations in EU -
in EU Member States)
Member States.
Specific dimension of the finished rolls (width x
1.3 x 75 m
length)
2.4 Placing on the market/ Application rules
For quality assurance, the geogrids RE500 series are regulated in accordance with European harmo-
nised standards and marked with a CE mark (or UKCA mark for the UK market) by the manufacturer.
In the EU/EFTA (excluding Switzerland) the placing of geogrids on the market is covered by Regulation
(EU) No. 305/2011 of 9 March 2011. For the product use the respective national provisions shall apply.
The product is packed and transported as roll and mainly marketed in Europe.
2.5 Base materials / Ancillary materials
Tensar® RE500 geogrids are manufactured from high-density polyethylene (HDPE). HDPE is a thermo-
plastic polymer known for its high strength-to-density ratio. It belongs to the group of polyolefins and
is partially crystalline and nonpolar. It is produced from the monomer ethylene. HDPE has little branch-
ing, giving it strong intermolecular forces and high tensile strength.
Raw material Unit Value
High-density polyethylene granules/pallets (HDPE) % 100
There is no biogenic carbon in the products.
The product does not contain substances from the “Candidate list of substances of very high concern
for authorisation” (SVHC).
Page | 3 Tensar International Limited – Tensar® RE510
2.6 Manufacturing
The manufacturing is located at Tensar Manufacturing Limited, 2 Sett End Road West, Blackburn, Lan-
cashire, BB1 2PU, United Kingdom. The geogrids are made from HDPE granulate. In the first step gran-
ulate is melted and then extruded. After this, the extruded sheet passes the punching process. De-
pending on the specific product the punches differ in size. The punched sheet is then stretched. The
result is the specific obround (uniaxial) structure of each geogrid. The products are rolled and then
packaged.
The manufacturing process is shown in the following figure:
Figure 1: Process flow chart of the production of Tensar® RE500
2.7 Packaging
Geogrids are rolled and banded twice with PP banding tape.
Page | 4 Tensar International Limited – Tensar® RE510
2.8 Reference Service Life (RSL)
The RSL of the soil reinforcement geogrid depends on the service life of the reinforced retaining wall,
slope or bridge abutment structure. The RE510 soil reinforcement geogrid is manufactured in accord-
ance with a Quality Management System compliant with BS EN ISO 9001:2008. The reference service
life of the product is up to 120 years. Further specification on the RSL of the product can be found in
the table below.
Characteristic Explanation
To be covered within 1 month after installa-
tion. Predicted to be durable for up to 100
Durability Statement (EN 13251, Annex B) years in natural soils with 4 ≤ pH ≤ 9 and soil
temperatures ≤25°C on the basis of the re-
sults of test method B.4.2 for 112 days.
Whilst the durability statement made in the
row above is the maximum allowed under
the constraints of the relevant CE marking
procedures as defined in the appropriate
hEN standards and/or EAD, Tensar are confi-
Additional Note to Durability Statement (EN 13251,
dent that no deterioration in properties will
Annex B)
occur for a period in excess of 120 years in
appropriate soil conditions and would ex-
pect no loss of in-situ performance when
stored outdoors for a period of 1 year prior
to installation.
2.9 Other Information
For further information on RE500 products please visit the official Tensar International Limited
webpage under the following link: www.tensar.co.uk
Page | 5 Tensar International Limited – Tensar® RE510
3. LCA: Calculation rules
3.1 Declared unit
In accordance with the PCR B 1 m2 of geogrid is chosen as the declared unit.
Product Unit Value
Declared Unit m2 geogrid 1
Unit weight g/m2 332
Conversion factor to 1 kg - 3.01
3.2 System boundary
The Environmental Product Declaration is a complete life cycle with a functional unit. It considers all
potential environmental impacts of the product from the cradle to the end of life.
The manufacturing phase includes the production or extraction of the source materials, the transport
to the respective production plant and the production of the geotextiles. All inputs (raw materials,
precursors, energy and auxiliary materials) as well as the by-products and waste are considered for all
life cycle phases. Finally, only production-related energy consumption (excluding administration and
social rooms) is considered.
The year 2020 represents the time reference for raw materials and electricity consumption. By defining
the scenarios (transport from production site to Utrecht and the choice of end-of-life scenarios) ac-
cording to specifications of the Dutch Environmental Database (NMD), the Netherlands is the relevant
geographical reference of this EPD. Due to manufacturing in Blackburn (Module A1-A3), the exact ge-
ographical reference area is the United Kingdom, but can also be considered representative for the
reference area Europe. Environmental effects such as the greenhouse effect can occur with a strong
spatial and temporal offset.
The following production steps are considered during the manufacturing phase:
• Extraction and processing of the raw materials (HDPE pre-compounded with UV and anti-
oxidant stabiliser packages)
• Transport to the production site
• Processing of the geogrids (extrusion, punching, stretching)
• Packaging (including packaging material)
• End-of-life (including transport)
Secondary fuels are not included in the production process and are therefore not considered. The
waste materials and quantities produced are included in the respective modules.
3.3 Estimates and assumptions
Almost all datasets chosen for the LCA refer to the EU as the geographic reference. Transport dis-
tances for all raw materials used (raw materials, operating materials, packaging) could be recorded. A
payload factor of 50% was used for all truck transports (suppliers, disposal transports and internal
transports), which corresponds to a full delivery and empty return trip. A data set for a non-specific
truck was used.
Page | 6 Tensar International Limited – Tensar® RE510
Tensar International Limited switched in 2020 to a 100% renewable wind energy. According to a wind
electricity portal, windbranche.de, 50% of wind power in UK is generated from onshore and 50% from
offshore wind parks. Based on this assumption an electricity data set was generated for the LCA calcu-
lation. No CO certificates were considered.
2
3.4 Cut-off criteria
All flows which influence is higher than 1% on the total mass, energy or environmental impact are in-
cluded in the LCA. It can be assumed that the neglected processes would have contributed less than
5% to the impact categories considered.
All process specific data could be determined and modelled by the use of generic data (EcoInvent 3.6)
The HDPE is bulk delivered in 24 tons batches – the pellets are blown into the silo. Therefore, there is
no packaging waste for the HDPE.
3.5 Period under review
The production data have been collected for the operating year 2020.
3.6 Data quality
For all processes primary data was collected and provided by Tensar International Limited. The primary
data refers to year 2020. For the data, which is not influenced by the manufacturer, generic data was
used. The secondary data was taken from the database EcoInvent (version 3.6). The database is main-
tained on a regular basis and thus meets the requirements of EN 15804 (background data not older
than 10 years). The power sources were chosen from data for the UK in 2020, in accordance with the
geographical and time representativeness. The data quality is very good, because all process specific
data could be documented and modelled by using the generic data.
RETHiNK EPD web application from the company NIBE was used to model the life cycle for the pro-
duction and disposal of the declared product systems. To ensure that the results are comparable, con-
sistent background data from the international database EcoInvent was used in the LCA (e.g. data rec-
ords on energy, transport, auxiliary materials, and supplies). Almost all consistent data sets contained
in the EcoInvent database are documented and can be viewed online.
3.7 Allocation
Allocations were avoided as far as possible. Tensar uses HDPE for several products as a raw material
and all PP residues, which occur during the manufacturing, are recycled. The residues are not
mandatorily used again for the product from which they originate. The recycled residues might be used
for products from another series.
For example: 5% residues of HDPE occur during the manufacturing of geogrid A. These 5% are recycled,
but due to operating conditions, it is possible that 4% is reused for geogrid A and 1% for geogrid B.
For this calculation it was assumed, that the generated punchout and the regrind material of a specific
geogrid is reused in a closed loop recycling for the analysed geogrid. This was done to avoid product
specific shifts of potential environmental impacts. It was also assumed that the recycled HDPE
substitutes virgin HDPE after a regranulation and that this does not imply any quality losses.
3.8 Comparability
In principle, a comparison or assessment of the environmental impacts of different products is only
possible if they have been prepared in accordance with EN 15804. For the evaluation of the
Page | 7 Tensar International Limited – Tensar® RE510
comparability, the following aspects have to be considered in particular: PCR used , functional or
declared unit, geographical reference, definition of the system boundary, declared modules, data
selection (primary or secondary data, background database, data quality), scenarios used for use and
disposal phases, and the life cycle inventory (data collection, calculation methods, allocations, validity
period). PCRs and general program instructions of different EPDs programs may differ. A comparability
needs to be evaluated. For further guidance see EN 15804+A2 (5.3 Comparability of EPD for
construction products) and ISO 14025 (6.7.2 Requirements for comparability).
Page | 8 Tensar International Limited – Tensar® RE510
4. LCA: Scenarios and additional technical information
The distance to the construction site (A4) was calculated according to the NMD (Nationale Milieu Da-
tabase (Dutch National Environmental Database)) method. Accordingly, the distance between the pro-
duction site in Blackburn and Utrecht was considered (900 km). As the mean of transportation truck
(unspecified) was chosen.
It is assumed that no activities for maintenance, repair, transport and replacement, refurbishment or
other material and energy flows take place during the RSL. Modules B1 to B3 are therefore assumed
to be zero. Product replacement (B4) and renovation (B5) only apply when the product is considered
in a lifespan (of a building, work, etc.). Operational water and energy use are not considered.
When installing the soil reinforcement geogrid, it is simply unrolled by hand on prepared layer of rein-
forced fill (granular/cohesive material) to the required reinforcement length, and then cut, often by
use of hand tools. Apart from rolling out, no further installation measures are necessary, which would
otherwise be required. RE layers are also installed manually vertically in Tensar Stratum (reinforcement
layers) applications. A reject or unused portion of 2-3% of the soil reinforcement geogrid is assumed
during the installation process (Module A5).
For C1 the process and amount of the generic dataset ‘Polyester weefsel’ (EN: polyester fabric) out of
chapter 22.46 Grondwapening en grondscheiding (EN: 22.46 Soil reinforcement and soil separation) of
the program DuboCalc with database version NMD version 1.8 - 5.01.14052018. In this generic dataset
0.0013 hrs of the process Gr.mach.hydr. (gemiddeld) (EN: Hydraulic excavator (average)) are stated for
module C1 (demolition).
For the end-of-life the NMD scenario PE/PP soil reinforcement (geotextile and geogrid) was chosen.
This scenario assumes that 25% of the geogrid remains in the subground, 70% are incinerated and 5%
are recycled.
Note: The transport distances of the waste are based on the standard waste scenarios of the NMD
Determination Method (SBK 2019): incineration 150 km/ recycling 50 km / landfill 100 km; vehicle:
truck, unspecific. For energy recovery, it is assumed that only fossil raw materials are substituted, con-
sidering the calorific values of the raw materials of the declared product and energy and thermal effi-
ciencies of 18% and 32%. According the EN 15804, loads are credited in A3 or C3 to C4 and benefits
are credited in module D.
For all transports, the environmental profile of a non-specific truck transport was used (conservative
assumption): The vehicle operates with diesel, and it provides a fleet average that includes different
lorry classes as well as EURO classes. This environmental profile contains data for transport, which is
calculated for an average load factor, including empty return trips (EcoInvent 3.6).
Page | 9 Tensar International Limited – Tensar® RE510
5. LCA: Results
The following tables show the results of the impact assessment indicators, resource use, waste and
other output streams. The results presented here refer to the declared specific product.
Disclaimer on ADP-e, ADP-f, WDP, ETP-fw, HTP-c, HTP-nc, SQP: The results of these environmental
impact indicators must be used with caution, as the uncertainties in these results are high or as there
is limited experience with the indicator.
Disclaimer on IR: This impact category mainly addresses the potential effect of low dose ionizing radi-
ation on human health in the nuclear fuel cycle. It does not consider effects due to possible nuclear
accidents and occupational exposures, nor does it consider radioactive waste disposal in underground
facilities. Potential ionizing radiation from soil, radon, and some building materials is also not measured
by this indicator.
Page | 10 Tensar International Limited – Tensar® RE510
Description of the system boundary
Construction process Benefits and loads beyond
Product stage Use stage End of life stage
stage the system boundaries
la ir e t a m w a Ry lp p u s t r o p s n a r T u n a M-g n ir u t c a f t r o p s n a r Tu n a m m o r-
f
o t r e r u t c a fe s u fo e c a lp n o it c u r ts n o
C
n o it a lla ts n -is s e c o r p e s U n ia M-e c n a n e t r ia p e R tn e m e c a lp e
R
r u fe R-n e m h s ib la n o it a r e p Oe s u y g r e n e la n o it a r e p Oe s u r e t a w e D- n o it c u r ts n o cn o itilo m e d
/
t r o p s n a r T e ts a Wg n is s e c o r p la s o p s iD e s u e R-y r e v o c e R- g n ilc y c e R- a itn e t o pl
A1 A2 A3 A4 A5 B1 B2 B3 B4 B5 B6 B7 C1 C2 C3 C4 D
X X X X X X X X MND MND MND MND X X X X X
X=Module declared | MND=Module not declared
Results of the LCA – Environmental impact: 1 m2 Tensar® RE510 (EN 15804+A2)
Parameter Unit A1 A2 A3 A4 A5 B1 B2 B3 C1 C2 C3 C4 D
Core environmental impact indicators
ADP-mm kg Sb-eqv. 5,95E-06 1,23E-06 1,08E-06 1,02E-06 3,07E-07 0,00E+00 0,00E+00 0,00E+00 1,04E-07 1,22E-07 8,00E-07 9,42E-09 -4,06E-07
ADP-f MJ 2,35E+01 3,89E-01 6,00E+00 6,08E-01 9,35E-01 0,00E+00 0,00E+00 0,00E+00 9,37E-01 7,26E-02 4,86E-01 2,08E-02 -7,49E+00
AP mol H+ eqv. 2,39E-03 1,29E-04 5,35E-04 2,34E-04 1,08E-04 0,00E+00 0,00E+00 0,00E+00 7,12E-04 2,79E-05 2,81E-04 7,68E-06 -4,30E-04
EP-fw kg PO4 eqv. 1,13E-05 2,85E-07 7,51E-06 4,07E-07 6,44E-07 0,00E+00 0,00E+00 0,00E+00 2,48E-07 4,86E-08 1,88E-06 1,58E-08 -9,86E-07
EP-m kg N eqv. 4,09E-04 2,56E-05 1,22E-04 8,24E-05 2,20E-05 0,00E+00 0,00E+00 0,00E+00 3,14E-04 9,84E-06 7,68E-05 4,65E-06 -1,13E-04
EP-t mol N eqv. 4,56E-03 2,87E-04 1,33E-03 9,09E-04 2,43E-04 0,00E+00 0,00E+00 0,00E+00 3,45E-03 1,09E-04 8,56E-04 2,82E-05 -1,25E-03
GWP-b kg CO2 eqv. 3,47E-03 1,03E-05 2,12E-04 1,86E-05 1,14E-04 0,00E+00 0,00E+00 0,00E+00 1,89E-05 2,22E-06 9,02E-05 9,48E-06 -2,77E-04
GWP-f kg CO2 eqv. 6,65E-01 2,65E-02 3,80E-01 4,03E-02 5,28E-02 0,00E+00 0,00E+00 0,00E+00 6,81E-02 4,82E-03 6,23E-01 1,23E-02 -4,10E-01
GWP-luluc kg CO2 eqv. 2,04E-04 1,54E-05 4,13E-05 1,48E-05 9,86E-06 0,00E+00 0,00E+00 0,00E+00 5,37E-06 1,76E-06 5,07E-05 4,35E-07 -2,12E-05
GWP-total kg CO2 eqv. 6,69E-01 2,65E-02 3,80E-01 4,04E-02 5,29E-02 0,00E+00 0,00E+00 0,00E+00 6,81E-02 4,82E-03 6,24E-01 1,23E-02 -4,10E-01
ODP kg CFC 11 eqv. 1,69E-08 5,65E-09 4,98E-08 8,90E-09 3,07E-09 0,00E+00 0,00E+00 0,00E+00 1,47E-08 1,06E-09 1,91E-08 2,72E-10 -4,97E-08
POCP kg NMVOC eqv. 2,22E-03 9,32E-05 4,67E-04 2,59E-04 9,96E-05 0,00E+00 0,00E+00 0,00E+00 9,49E-04 3,10E-05 2,30E-04 1,08E-05 -4,49E-04
WDP m3 world eqv. 5,34E-01 1,34E-03 3,46E-01 2,18E-03 2,75E-02 0,00E+00 0,00E+00 0,00E+00 1,26E-03 2,60E-04 3,18E-02 8,92E-04 -5,48E-02
Additional environmental impact indicators
ETP-fw CTUe 3,72E+00 3,49E-01 1,60E+00 5,42E-01 4,28E-01 0,00E+00 0,00E+00 0,00E+00 5,65E-01 6,48E-02 7,84E+00 2,22E-02 -5,55E-01
HTP-c CTUh 1,75E-10 1,28E-11 2,08E-10 1,76E-11 1,62E-11 0,00E+00 0,00E+00 0,00E+00 1,97E-11 2,10E-12 1,19E-10 5,81E-13 -3,27E-11
HTP-nc CTUh 4,07E-09 3,45E-10 2,46E-09 5,93E-10 3,02E-10 0,00E+00 0,00E+00 0,00E+00 4,85E-10 7,09E-11 2,48E-09 1,44E-11 -5,45E-10
IRP kBq U235 eqv. 1,57E-02 1,70E-03 3,82E-03 2,55E-03 7,85E-04 0,00E+00 0,00E+00 0,00E+00 4,02E-03 3,04E-04 1,99E-03 8,15E-05 -2,83E-03
disease 1,98E-08 1,22E-09 3,86E-09 3,63E-09 9,42E-10 0,00E+00 0,00E+00 0,00E+00 1,89E-08 4,33E-10 2,28E-09 1,45E-10 -1,89E-09
PM incidence
SQP - 7,68E-01 1,83E-01 4,82E-01 5,28E-01 6,77E-02 0,00E+00 0,00E+00 0,00E+00 1,20E-01 6,30E-02 1,79E-01 4,92E-02 -1,30E-01
ADP-mm= Abiotic depletion potential for non-fossil resources | ADP-f=Abiotic depletion for fossil resources potential | AP= Acidification potential, Accumulated Exceedance | EP-fw = Eutrophication potential, fraction of nutrients reaching
freshwater end compartment | EP-m= Eutrophication potential, fraction of nutrients reaching marine end compartment| EP-T= Eutrophication potential, Accumulated Exceedance | GWP-b=Global Warming Potential biogenic | GWP-
f=Global Warming Potential fossil fuels | GWP-luluc=Global Warming Potential land use and land use change |GWP-total=Global Warming Potential total| ODP=Depletion potential of the stratospheric ozone layer |POCP=Formation
potential of tropospheric ozone | WDP=Water (user) deprivation potential, deprivation- weighted water consumption | ETP-fw=Potential Comparative Toxic Unit for ecosystems | HTP-c=Potential Toxic Unit for Humans toxicity, cancer |
HTP-nc= Potential Toxic Unit for humans, non-cancer | IRP=Potential Human exposure efficiency relative to U235, human health | PM=Potential incidence of disease due to Particulate Matter emissions | SQP=Potential soil quality index
Page | 11 Tensar International Limited – Tensar® RE510
Results of the LCA – Resource and environmental information: 1 m2 Tensar® RE510 (EN 15804+A2)
Parameter Unit A1 A2 A3 A4 A5 B1 B2 B3 C1 C2 C3 C4 D
PERE MJ 3,94E-01 7,99E-03 9,50E+00 7,61E-03 2,99E-01 0,00E+00 0,00E+00 0,00E+00 5,07E-03 9,09E-04 4,92E-02 3,69E-04 -3,36E-02
PERM MJ 0,00E+00 0,00E+00 0,00E+00 0,00E+00 0,00E+00 0,00E+00 0,00E+00 0,00E+00 0,00E+00 0,00E+00 0,00E+00 0,00E+00 0,00E+00
PERT MJ 3,94E-01 7,99E-03 9,50E+00 7,61E-03 2,99E-01 0,00E+00 0,00E+00 0,00E+00 5,07E-03 9,09E-04 4,92E-02 3,69E-04 -3,36E-02
PENRE MJ 1,27E+01 4,13E-01 6,50E+00 6,46E-01 6,30E-01 0,00E+00 0,00E+00 0,00E+00 9,95E-01 7,71E-02 5,16E-01 2,21E-02 -7,62E+00
PENRM MJ 1,25E+01 0,00E+00 1,19E-01 0,00E+00 3,79E-01 0,00E+00 0,00E+00 0,00E+00 0,00E+00 0,00E+00 0,00E+00 0,00E+00 -6,44E-01
PENRT MJ 2,52E+01 4,13E-01 6,62E+00 6,46E-01 1,01E+00 0,00E+00 0,00E+00 0,00E+00 9,95E-01 7,71E-02 5,16E-01 2,21E-02 -8,26E+00
SM Kg 0,00E+00 0,00E+00 0,00E+00 0,00E+00 0,00E+00 0,00E+00 0,00E+00 0,00E+00 0,00E+00 0,00E+00 0,00E+00 0,00E+00 0,00E+00
RSF MJ 0,00E+00 0,00E+00 0,00E+00 0,00E+00 0,00E+00 0,00E+00 0,00E+00 0,00E+00 0,00E+00 0,00E+00 0,00E+00 0,00E+00 0,00E+00
NRSF MJ 0,00E+00 0,00E+00 0,00E+00 0,00E+00 0,00E+00 0,00E+00 0,00E+00 0,00E+00 0,00E+00 0,00E+00 0,00E+00 0,00E+00 0,00E+00
FW M3 8,05E-03 5,31E-05 8,16E-03 7,41E-05 5,20E-04 0,00E+00 0,00E+00 0,00E+00 4,83E-05 8,85E-06 9,35E-04 2,17E-05 -7,77E-04
HWD Kg 2,85E-06 1,03E-06 9,88E-06 1,54E-06 4,96E-07 0,00E+00 0,00E+00 0,00E+00 2,55E-06 1,84E-07 9,26E-07 3,17E-08 -8,09E-06
NHWD Kg 2,11E-02 1,11E-02 3,57E-02 3,86E-02 6,20E-03 0,00E+00 0,00E+00 0,00E+00 1,11E-03 4,61E-03 1,20E-02 8,32E-02 -3,61E-03
RWD Kg 1,40E-05 2,59E-06 4,89E-06 3,99E-06 8,36E-07 0,00E+00 0,00E+00 0,00E+00 6,51E-06 4,77E-07 1,75E-06 1,24E-07 -3,72E-06
CRU Kg 0,00E+00 0,00E+00 0,00E+00 0,00E+00 0,00E+00 0,00E+00 0,00E+00 0,00E+00 0,00E+00 0,00E+00 0,00E+00 0,00E+00 0,00E+00
MFR Kg 0,00E+00 0,00E+00 1,66E-04 0,00E+00 5,04E-04 0,00E+00 0,00E+00 0,00E+00 0,00E+00 0,00E+00 1,66E-02 0,00E+00 0,00E+00
MER Kg 0,00E+00 0,00E+00 0,00E+00 0,00E+00 0,00E+00 0,00E+00 0,00E+00 0,00E+00 0,00E+00 0,00E+00 0,00E+00 0,00E+00 0,00E+00
EE MJ 0,00E+00 0,00E+00 4,28E-02 0,00E+00 0,00E+00 0,00E+00 0,00E+00 0,00E+00 0,00E+00 0,00E+00 0,00E+00 0,00E+00 4,41E+00
PERE=Use of renewable primary energy excluding renewable primary energy resources used as raw materials | PERM= Use of renewable primary energy resources used as raw materials | PERT=Total use of renewable primary energy
resources | PENRE= Use of non-renewable primary energy excluding non-renewable primary energy resources used as raw materials | PENRM= Use of non-renewable primary energy resources used as raw materials | PENRT= Total use of
non-renewable primary energy resources | SM=Use of secondary material | RSF=Use of renewable secondary fuels | NRSF=Use of non-renewable secondary fuels | FW=Use of fresh water | HWD=Hazardous waste disposed | NHWD=Non-
hazardous waste disposed | RWD=Radioactive waste disposed | CRU=Components for re-use | MFR=Materials for recycling | MER=Materials for energy recovery | EE=Exported energy
Results of the LCA – Environmental impact, optional : 1 m2 Tensar® RE510 (Set 1 of the NMD determination method (version 1.0; July 2020))
Parameter Unit A1 A2 A3 A4 A5 B1 B2 B3 C1 C2 C3 C4 D
ADP-e Kg Sb 5,95E-06 1,23E-06 1,08E-06 1,02E-06 3,07E-07 0,00E+00 0,00E+00 0,00E+00 1,04E-07 1,22E-07 8,00E-07 9,42E-09 -4,06E-07
ADP-f Kg Sb 1,12E-02 1,85E-04 3,22E-03 2,94E-04 4,57E-04 0,00E+00 0,00E+00 0,00E+00 4,45E-04 3,51E-05 2,59E-04 1,01E-05 -3,97E-03
GWP Kg CO2 eqv. 6,39E-01 2,63E-02 3,75E-01 4,00E-02 5,18E-02 0,00E+00 0,00E+00 0,00E+00 6,74E-02 4,78E-03 6,23E-01 1,05E-02 -4,04E-01
ODP Kg CFC-11 eqv. 1,77E-08 4,53E-09 4,40E-08 7,10E-09 2,83E-09 0,00E+00 0,00E+00 0,00E+00 1,17E-08 8,47E-10 1,91E-08 2,18E-10 -4,39E-08
POCP Kg Ethene eqv. 6,09E-04 1,43E-05 8,66E-05 2,41E-05 2,29E-05 0,00E+00 0,00E+00 0,00E+00 6,86E-05 2,88E-06 2,22E-05 2,39E-06 -8,37E-05
AP Kg SO2 eqv. 1,99E-03 1,05E-04 4,32E-04 1,76E-04 8,87E-05 0,00E+00 0,00E+00 0,00E+00 5,08E-04 2,10E-05 2,19E-04 5,83E-06 -3,41E-04
EP Kg PO43- eqv. 1,86E-04 1,33E-05 6,90E-05 3,45E-05 1,04E-05 0,00E+00 0,00E+00 0,00E+00 1,15E-04 4,13E-06 3,57E-05 2,35E-06 -4,41E-05
HTP kg 1.4 DB 1,04E-01 9,66E-03 1,27E-01 1,68E-02 9,20E-03 0,00E+00 0,00E+00 0,00E+00 2,50E-02 2,01E-03 4,54E-02 8,62E-04 -2,45E-02
FAETP kg 1.4 DB 1,96E-03 2,49E-04 8,94E-04 4,92E-04 2,07E-04 0,00E+00 0,00E+00 0,00E+00 3,47E-04 5,87E-05 2,33E-03 8,97E-04 -2,94E-04
MAETP kg 1.4 DB 6,28E+00 9,32E-01 2,52E+00 1,77E+00 5,84E-01 0,00E+00 0,00E+00 0,00E+00 1,21E+00 2,11E-01 6,79E+00 8,96E-01 -1,19E+00
TETP kg 1.4 DB 4,12E-04 4,15E-05 4,22E-04 5,95E-05 3,19E-05 0,00E+00 0,00E+00 0,00E+00 4,11E-05 7,11E-06 1,16E-04 1,49E-06 -8,13E-05
ADP-e= Abiotic depletion potential for elements | ADP-f= Abiotic depletion for fossil resources potential | GWP=Global Warming Potential | ODP=Depletion potential of the stratospheric ozone layer | POCP= Formation potential of tropo-
spheric ozone | AP= Acidification potential, Accumulated Exceedance | EP= Eutrophication potential, Accumulated Exceedance | HTP= human-toxicological effects | FAETP= ecotoxicological effects, aquatic (freshwater) | MAETP= ecotoxi-
cological effects, aquatic (marine water) | TETP= ecotoxicological effects, terrestrial
Page | 12 Tensar International Limited – Tensar® RE510
6. LCA: Interpretation
As shown in the figure below, raw material supply (A1) dominates in most environmental core
indicators, often followed by the production process (A3). In some environmental core indicators
demolition phase (C1) has a great impact. However, C1 is strongly dependent on the assumption (here
diesel consumption of a construction site vehicle). The highest influence on the Global Warming
Potential have row material supply (A1), waste processing (C3), and production process (A3).
Transports (A2, A4, C2) have rather a minor impact within all core indicators.
100%
80%
60%
40%
20%
0%
-20%
-40%
ADP-mm ADP-f AP EP-fw EP-m EP-T GWP-total ODP POCP WDP
A1 A2 A3 A4 A5 C1 C2 C3 C4 D
Figure: Tensar® RE510 - Impact of the individual modules on the environmental core indicators
The MKI (Dutch: Milieukostenindicator) value calculated based on set 1 of the NMD determination
method amounts to 0.122.
The data quality can be classified as good overall. All relevant process-specific data could be collected
in the operational data collection. Consistent data sets from the EcoInvent database were available for
almost all inputs and outputs. The background data meet the requirements of EN 15804, and the pro-
duction data were recorded for the 2020 operating year. The quantities of raw materials and supplies
used as well as energy consumption were recorded for the entire operating year.
Page | 13 Tensar International Limited – Tensar® RE510
7. Requisite evidence
In 2020, RE570 was tested concerning its leaching behavior using the trough method. Due to this
method the institute “Prüftechnik Z+L” could determine the direct environmental impacts to the local
environment (soil and groundwater). In accordance with the criteria of the German Federal Soil Pro-
tection and Contaminated Sites Ordinance (Bundesbodenschutz- und Altlastenverordnung) the envi-
ronmental soundness of the geogrid could be confirmed. This result can be transferred to all the other
types of geogrids referring to the product series RE500, and therefore to the RE510.
Page | 14 Tensar International Limited – Tensar® RE510
8. References
CML-IA April 2013 – Charakterisierungsfaktoren entwickelt durch Institut of Environmental Sciences
(CML): Universität Leiden, Niederlande - http://www.cml.leiden.edu/software/data-cmlia.html
Donndorf, R., Kahle H., Müller, G., Philipp H-J., Taschow, H-J., Wolf, O. (1973): Werkstoffeinsatz und
Korrosionsschutz in der chemischen Industrie. VEB Deutscher Verlag für Grundstoffindustrie Leipzig.
European Commission Joint Research Centre Institute for Prospective Technological Studies (JCR
2014): End-of-waste criteria for waste plastic for conversion, Seville, 2014, doi:10.2791/13033
Klöpffer, W., Grahl B.: Ökobilanz (LCA) – Ein Leitfaden für die Ausbildung und Beruf, Wily-VCH Ver-
lag, Weinheim, 2007
Rosauer, V. (2010): Abschätzung der herstellungsbedingten Qualität und Lebensdauer von Asphalt-
deckschichten mit Hilfe der Risikoanalyse (Estimation of the production-related quality and service
life of asphalt wearing courses with the aid of risk analysis). Technischen Universität Darmstadt, 2010
Stichting Bouwkwaliteit (SBK) – Foundation for Building Quality; “Determination Method: Environmen-
tal Performance of Buildings and Civil Engineering Works”
NMD determination method: Stichting Nationale Milieudatabase; Bepalingsmethode Milieuprestatie
Bouwwerken; Version 1.0; July 2020; Berekeningswijze voor het bepalen van de milieuprestatie van
bouwwerken gedurende hun gehele levensduur, gebaseerd op de EN 15804.
Windbranche.de – Das Branchenportal rund um die Windenergie. Wind power and electricity genera-
tion in Great Britain: https://www.windbranche.de/wind/windstrom/windenergie-grossbritannien,
last accessed 19 July 2021.
Standards and laws
ISO 14040:2006, Environmental management - Life cycle assessment - Principles and framework
ISO 14044:2006, Environmental management - Life cycle assessment - Requirements and guidelines
ISO 14025:2006: Environmental labels and declarations — Type III environmental declarations —
Principles and procedures EN 13249
EN 15804:2012+A2:2019 Sustainability of construction works — Environmental Product Declarations
— Core rules for the product category of construction products
PCR A: General Program Category Rules for Construction Products from the EPD program Kiwa-Eco-
bility Experts, R.0_2021-07-16
PCR B: Product Category Rules (PCR) from the Kiwa-Ecobility Experts EPD program: “Geosynthetic
products”, edition 2022-02-08 (draft)
Page | 15 Tensar International Limited – Tensar® RE510
Publisher Mail DE.Ecobility.Ex-
Kiwa-Ecobility Experts perts@kiwa.com
Voltastr. 5 Web https://www.kiwa.com/de/de
13355 Berlin /themes/ecobility-ex-
Germany perts/ecobility-experts/
Programme operator Mail DE.Ecobility.Ex-
Kiwa-Ecobility Experts perts@kiwa.com
Voltastr. 5 Web https://www.kiwa.com/de/de
13355 Berlin /themes/ecobility-ex-
Germany perts/ecobility-experts/
Author of the Life Cycle Tel. +49 (0) 30 467761-43
Assessment Fax. +49 (0) 30 467761-10
Kiwa GmbH Mail DE.Nachhaltigkeit@kiwa.com
Voltastr.5
13355 Berlin Web https://www.kiwa.com/
Germany
Owner of the declaration Tel. +44 (0) 1254 262 431
Tensar International Limited Fax. +44 (0) 1254 266 867
Units 2-4 Cunningham Court Mail info@tensar-internatio-
Shadsworth Business Park nal.com
Blackburn, United Kingdom Web www.tensar.co.uk
Page | 16 Tensar International Limited – Tensar® RE510
