ENVIRONMENTAL PRODUCT DECLARATION
as per ISO 14025 and EN 15804+A2
Owner of the Declaration
Programme holder Institut Bauen und Umwelt e.V. (IBU)
Publisher Institut Bauen und Umwelt e.V. (IBU)
Declaration number EPD­HIL­20220123­IBA1­EN
Issue date 20.06.2022
Valid to 19.06.2027
Hilti HIT­HY 270
HILTI AG
www.ibu-epd.com | https://epd-online.com
Umwelt Produktdeklaration Name des Herstellers – Name des Produkts
1. General Information
HILTI AG HIT­HY 270
Programme holder Owner of the declaration
IBU – Institut Bauen und Umwelt e.V. Hilti AG
Hegelplatz 1 Feldkircher Str. 100
10117 Berlin FL­9494 Schaan
Germany Liechtenstein
Declaration number Declared product / declared unit
EPD­HIL­20220123­IBA1­EN The declared product is a HILTI injectable mortar HIT­
HY 270. The declared unit is one kilogram of reaction
resin product in the mixing ratio of the two components
necessary for processing. The packaging is also
included in the calculation. The declared unit is stated
in [kg].
This declaration is based on the product Scope:
category rules: This document refers to the injectable mortar HIT­HY
Reaction resin products, 11.2017 270 with its packaging. For the compilation of the life
(PCR checked and approved by the SVR) cycle assessment, specific data were collected from
the factory in Kaufering, Germany, of the HILTI AG.
Data from the year 2018 are used, which correspond to
Issue date
the annual average.
20.06.2022
The owner of the declaration shall be liable for the
Valid to
underlying information and evidence; the IBU shall not
19.06.2027
be liable with respect to manufacturer information, life
cycle assessment data and evidences.
The EPD was created according to the specifications
of EN 15804+A2. In the following, the standard will be
simplified as EN 15804.
The owner of the declaration shall be liable for the
underlying information and evidence; the IBU shall not
be liable with respect to manufacturer information, life
cycle assessment data and evidences.
The EPD was created according to the specifications
of EN 15804+A2. In the following, the standard will be
simplified as EN 15804.
Verification
The standard EN 15804 serves as the core PCR
Independent verification of the declaration and data
according to ISO 14025:2011
Dipl. Ing. Hans Peters internally x externally
(chairman of Institut Bauen und Umwelt e.V.)
Dr. Alexander Röder Matthias Klingler
(Managing Director Institut Bauen und Umwelt e.V.)) (Independent verifier)
2. Product
2.1 Product description/Product definition Mixing the two components A and B in the static mixer
initiates the curing (hardening) reaction of both binder
The declared product of HIT­HY 270 is a two­ systems. During the curing phase, a very strong bond
component system. is formed between the organic and inorganic binder
matrix.
The resin component (component A) comprises a resin The hybrid system formed during cement and resin
based on methacrylate as well as mineral and cement­ curing results in a cross­linked duromer with desired
like fillers. The curing agent component (component B) design properties (high bond strengths within short
comprises of peroxide hardener, water and mineral curing time) and particular long­term stability.
fillers. Composite foils are used for the two­component foil
pack of HIT­HY 270. This kind of packaging serves the
2 Environmental Product Declaration Hilti AG – HIT­HY 270
following purposes: waste volume reduction, easy Shelf life of 12 months:
storage and transport, less packaging material. Substrate temperature during installation +5 to +40 °C
Through legislation and increased public awareness (internal method).
users have increasingly become discerned towards the
use of styrene and other highly volatile components Working time:
with their resulting unpleasant odour and low flash 0 to +4 °C 10 min (hollow bricks only)
point (flammability). > 4 to +9 °C 10 min
The reaction resins used in all Hilti hybrid adhesives > 9 to +19 °C 7 min
contain no styrene, are practically odourless and have > 19 to +29 °C 4 min
a considerably higher flash point, i.e. higher than 100 > 29 to +40 °C 1 min
°C in comparison to 34 °C for styrene­based products.
HIT­HY 270 is the ultimate performance injectable Curing time:
hybrid mortar with approvals for fastenings in all 0 to +4 °C 4 h (hollow bricks only)
masonry materials. > 4 to +9 °C 2,5 h
For the placing of the product on the market in the > 9 to +19 °C 1,5 h
European Union European Free Trade Association > 19 to +29 °C 30 min
EU/EFTA) (with the exception of Switzerland) the > 29 to +40 °C 20 min
Regulation (EU) No. 305/2011 (CPR) applies. The
product needs a declaration of performance taking into 2.4 Delivery status
consideration the following European Technical The product Hilti HIT­HY 270 is available in foil­
Approvals packages with a total of 330 ml and 500 ml injectable
ETA 13/1036 mortar in the corresponding mixing ratio.
ETA 19/0160
and the CE­marking. For the application and use the 2.5 Base materials/Ancillary materials
respective national provisions apply. Hilti HIT­HY 270 is supplied in the form of a dual
component film­wrapped pack comprising a resin
2.2 Application component and a curing agent component at a volume
Hilti HIT­HY 270 serves for safely securing of threaded ratio of 3:1. The mixing ratio of resin and curing agent
rods and masonry. components is automatically set during the injection
process. Product curing commences directly after the
Hilti HIT­HY 270 is a component of the Hilti SAFEset components are mixed.
concept. Hilti SAFEset is an approved system which
makes anchor installation an easier, safer and faster The product reviewed in this EPD contains the
process. It significantly improves the robustness of following component volumes:
fastening and dramatically reduces the possibilities of
error during installation. As part of SAFEset HIT­HY Resin component:
270 can be installed with approved Hilti Hollow Drill Methacrylate resin mixture: 40 to 50% by weight
bits and vacuum cleaners that drill and clean the hole Mineral fillers: 30 to 40% by weight
in one step for virtually dust­free installation. When use Cement: 10 to 20% by weight
with Hilti HIT­Z rod as part of the SAFEset, no cleaning Other: < 5% by weight
of the borehole is required. The use of Hilti HDE­22
dispenser with Volume Calculator app leads to no Curing agent component:
under or over fill, reducing underfilling related risks and Mineral fillers: 50 to 60% by weight
minimizing mortar wastage. Water: 20 to 30% by weight
Dibenzoyl peroxide: 5 to 10% by weight
2.3 Technical Data Other: ~ 5% by weight
This product article contains substances listed in the
Constructional data REACH candidate list (date: 28.04.2022) exceeding
Name Value Unit 0.1 percentage by mass: yes, boric acid, less than 1
Density EN ISO 1183­1 1670 kg/m3 percent by mass (EC 233­139­2, CAS 10043­35­3).
Compressive strength
63 N/mm^2
(Tcure=120h) EN ISO 604 This product contains other CMR substances in
Elastic modulus (pressure) EN categories 1A or 1B which are not on the candidate
1300 N/mm^2
ISO 604 list, exceeding 0.1 percentage by mass: yes, boric acid
Tensile shear strength acc. to DIN not is classified as Repr. 1B, H360FD.
N/mm2
EN 14293 relevant
Tensile bond strength acc. to DIN not Biocide products were added to this construction
N/mm2
EN 14293 relevant product or it has been treated with biocide products
(this then concerns a treated product as defined by the
(EU) Ordinance on Biocide Products No. 528/2012):
Hilti HIT-HY 270 displays the following no.
characteristics:
2.6 Manufacture
Performance data of the product in accordance with Most raw materials are sourced from Europe. The
the declaration of performance with respect to its transport is exclusively by truck for the European raw
essential characteristics according to materials, and by truck and by ship for the others.
ETA 13/1036 Chemical mortars are usually two­component systems
ETA 19/0160 consisting of a binder and a hardener. One of the base
components of the binder is the reactive resin which in
the case of HIT­HY 270 is produced in Kaufering. The
3 Environmental Product Declaration Hilti AG – HIT­HY 270
resin production process is a chemical reaction of the 1) For safe handling the precautionary measures
corresponding educts to a basic resin with subsequent described in the SDS (e.g. hand and eye protection)
mixing of the basic resin with different reactive diluents must be adhered to
to a reactive resin. This process is controlled and 2) Insert the cartridge into the black cassette
monitored by process control technology. 3) Screw on the mixing nozzle
The production of chemical mortars consists of a 4) Put the cassette into the dispenser system
mixing process and a filling process of the respective 5) Discard the first trigger pulls
single components (binder and hardener) and their 6) Fill 2/3 of the borehole with mortar
subsequent union to a two­component system 7) Set the fixing element
(container). Here as well process control technology is
used to weigh and mix solid and liquid compounds After mixing the components and squeezing the mortar
according to specification. In the next step both well­ into the borehole the fixing element has to be set within
mixed components run through an automized filling the working time mentioned in Instructions for Use.
line in which each of the processed masses is filled After the curing time, described as well in Instructions
into a tubular foil bag. Finally the single components for Use, the mortar is ready to take up loads.
are united in one container. The two­pack foil bags are
packed into cardboard boxes and then finally shipped. 2.9 Packaging
The manufacturing plant of HIT­HY 270, Hilti GmbH Hilti HIT­HY 270 is supplied in the form of a 2­foil­pack
Industriegesellschaft für Befestigungstechnik, Hiltistr. system and thus leads to very little waste remaining
6, 86916 Kaufering, Germany, is certified according to after use on the construction site. After curing, the
ISO 9001. The guideline defines international product can be disposed of with household waste. Full
standards for quality and process management. or only partially emptied cartridges must be disposed
The following flowcharts illustrate the underlying of as special waste in accordance with official
production process regulations.
The outer packaging consisting of plastic foil and
cardboard boxes designed according to the product
size can be recycled. Packaging contaminated by the
product must be disposed in a safe manner in
accordance with local/national regulations.
For this EPD, the declared packaging is a weighted
meanvalue of all available packaging sizes. This
results in a 144 g packaging composed of 69 g of
plastic, 69 g of paper and cardboard, 5 g of aluminium.
2.10 Condition of use
During the installation the temperature of the base
material must be between +5°C and +40°C for solid
Illustration: Production process of the reaction clay bricks and between ­5°C and +40°C for other
resin mixture base materials. The temperature of the product should
be between +5 and +25 °C during storage +5 and
40°C during usage. Hilti literature and official approvals
must always be considered. The two components of
HIT­HY 270 are only for use in combination with the
defined volume ratio and under these conditions
mentioned above to build up a cross­linked filled
duromer.
2.11 Environment and health during use
Refer to the Safety Data Sheet (SDS) for detailed
information on handling, storage as well as first aid,
firefighting and accidental release measures and
disposal considerations. Following the given
instructions helps to minimize the risk for health and
Illustration: Production process of the packaging environment.
2.7 Environment and health during 2.12 Reference service life
manufacturing Hilti HIT­HY 270 is exposed to a wide variety of
The manufacturing plant of HIT­HY 270,Hilti GmbH environmental factors during the use phase. The
Industriegesellschaft für Befestigungstechnik, Hiltistr. anticipated Reference Service Life depends on the
6, 86916 Kaufering, Germany, is certified according to specific installation situation and the product exposure
ISO 14001 which defines international standards for scenario. The main factors influencing the period of
sustainable environmental management. The use involve weathering as well as mechanical loads
production site is also certified in accordance with DIN and chemical exposure.
EN ISO 50001 Energy Management Systems.
2.8 Product processing/Installation 2.13 Extraordinary effects
The product is delivered with Instructions for Use
explaining the basic steps for installation: Fire
Even without any special fire safety features the
Injection Systems comply with at least the
4 Environmental Product Declaration Hilti AG – HIT­HY 270
requirements of the DIN EN 13501­1 standard for fire
classes E and Efl. As cross­linked methacrylate resins Water
do not melt or drip, the resins do not contribute The cured product is chemically inert and insoluble in
towards spreading fire. Apart from the common water.
combustion produces carbon monoxide and carbon
dioxide, fire gases can contain traces of methyl Mechanical destruction
methacrylate, esters, alcohol, and hydrocarbons. Due It is recommended to use dust protection during
to the quantities used, they only have a subordinate demolition of the cured chemical anchor.
influence on the fire characteristics of a building
structure in which they have been installed and 2.14 Re-use phase
therefore the anchorage is classified as A1 in the ETA. The product cannot be re­used. After usage the
product can be removed by demolition.
Fire protection 2.15 Disposal
Name Value Uncured Hilti HIT­HY 270 can be disposed of
Building material class E/Efl according to the European waste code 08 04 09* or 20
No 01 27*. The built­in cured anchor can be disposed as
performen construction waste for which the European waste code
Burning droplets
ce 17 01 01 applies.
assessed
No
performen 2.16 Further information
Smoke gas development
ce Further information is available on request under
assessed anchor.hse@hilti.com and on the Hilti website:
www.hilti.group
3. LCA: Calculation rules
3.1 Declared Unit A5 – Installation­Construction
The declared product is a HILTI injection mortar HIT­ electricity consumption for drilling and
HY 270. The declared unit refers to one kilogram of injectingElectricity consumption for injecting (in case of
reaction resin product in the required mixing ratio of injection with electrical dispenser).
the two components. The packaging of 0,144 kg/kg of Production of the construction losses.
product is also included in the calculation. The Provision and end­of­life of tools and accessories for
following table shows the data of the declared unit. injectable mortars (manual or electrical dispenser with
or without battery and with cartridge holder).
Declared unit End­of­life of hazardous construction losses and
Name Value Unit packaging (uncured mortar and soiled packaging) and
Declared unit 1 kg non­hazardous construction losses (cured mortar and
unsoiled packaging): including waste transportation,
processing and disposal.
C1 – Deconstruction/demolition
3.2 System boundary Diesel for building demolition.
The type of the EPD is cradle to grave. The following C2 – Transport (to waste processing)
information modules are defined as system boundaries Transportation to waste processing facility.
in this study: C4– Waste disposal
Treatment and disposal of plastic to sanitary landfill.
A1 – Raw material supply:
Production and packaging of the raw materials to be For the environmental impact, the use of green
supplied to the manufacturer. All processes are electricity (stage A3) was calculated taking into
included from cradle to gate. account the residual electricity mix for the remaining
A2 – Transport (to manufacturing site): electricity. The proportion of the electricity demand
Transportation of all the raw materials and their covered by green electricity in the total electricity
packaging between their production site and the demand is 100%.
manufacturing site, for all transport modes (sea, road).
A3 – Manufacturing: 3.3 Estimates and assumptions
Production, supply and use of energy sources at the In general, background data and elecricity mixes are
manufacturing sites (electricity, biomass and natural chosen and calculated country­specifically for the
gas). Green electricity from wind turbines is production processes. In some cases, assumptions
considered for the whole manufacturing process. were made because of a lack of primary or secondary
Production and transport of production losses, final data, in particular for the following aspects:
product packaging and other inputs.  The synthesis way of raw materials which
End­of­life of production waste (hazardous, non­ were not available on the Ecoinvent database
hazardous and recyclable), production losses and raw
were used to reconstructed these material's
material packaging, including waste and losses
impact
transportation, processing and disposal.
 Some raw material's packaging composition
A4 – Transport (to construction site)
Transportation of packaged products from the and transportation distances were estimated
manufacturing site to the construction site, including  The energy consumption for production of the
potential in­betweens (retailer, workshop, etc.). current product (HIT­HY 270) was assimilated
5 Environmental Product Declaration Hilti AG – HIT­HY 270
to the energy consumption measured on the up­to­date. The mass of the different components of
production line of another Hilti product, which the reactive resin mixture come from the information in
the recipe. The data quality is classified as appropriate.
has a very similar manufacturing process
 Estimations were made to calculate the
3.7 Period under review
energy consumption during installation
Data from the year 2018 are used, which correspond
 The transportation scenario to building site is to the annual average.
based on french transportation companies
statistics. 3.8 Allocation
The energy for manufacturing (A3) is supposed to be
the same as for another HITLI product, which
consumptions were measured on production line. No
3.4 Cut-off criteria
allocation was used for this stage.
All information modules considered were included in
The used operating tools (stage A5), which are Hilti's
the calculation in such detail that all requirements of
manual or electrical dispenser can be used to inject the
/EN 15804/ are met. The consumption of additional
HIT­HY 270 as well as other Hilti products. The part of
inputs such as lubricants, oils or solvents used for
the dispenser's impact allocated to the current product
manufacture is less than 5% by weight and therefore
is based on the estimated total mass of injected
falls below the cut­off criterion of the total calculation.
product each dispenser can be used for. This can be
considered as a mass allocation.
3.5 Background data
The source for background data for the LCA
3.9 Comparability
calculations is the ecoinvent 3.8 database.
Basically, a comparison or an evaluation of EPD data
is only possible if all the data sets to be compared
3.6 Data quality
were created according to EN 15804 and the building
For the compilation of the life cycle assessment,
context, respectively the product­specific
specific data were collected from the factory Kaufering,
characteristics of performance, are taken into account.
in Germany, of the HILTI AG from the year 2018. The
background data from the ecoinvent 3.8 database
The used background database is given by ecoinvent
used was updated in the year 2021 and thus of highly
3.8 database, to which this study refers.
4. LCA: Scenarios and additional technical information
Characteristic product properties Material loss 0.07 kg
Information on biogenic Carbon Hazardous waste (soiled
0,063 kg
The declared product contains 69 g of paper and packaging)
cardboard (outer packaging and user manual). Since Non­hazardous waste (unsoiled
0,080 kg
only this materials contain biogenic carbon, in addition packaging)
to a neglectable part contained in the raw material's
packaging, all the biogenic carbon capture and release
were cancelled to simplify the model.
The cancelled emission corresponds to 0,009 kg of End of life (C1-C4)
biogenic carbon (0,0331 kg of CO2) for a cancelled Name Value Unit
capture of 0,017 kg of biogenic carbon (0,0618 kg of Fuel for building demolition 0,0437 MJ
CO2). Distance to sanitary landfill 50 km
Landfilling 1 kg
The following scenarios were considered for the LCA
calculations:
Transport to the building site (A4)
Name Value Unit
Transport distance 900 km
lorry 16­
32
Vehicle type ­
metric
ton
Effective load 21 t
Maximum capacity 24 t
Consumption when unloaded 0,25 L/km
Consumption at fill capacity 0,38 L/km
Empty return rate 14 %
Effective consumption 0,019 L/tkm
Installation into the building (A5)
Name Value Unit
Electricity consumption 0.000306 kWh
Uncured mortar loss 0,04 kg
Cured mortar loss 0,03 kg
6 Environmental Product Declaration Hilti AG – HIT­HY 270
5. LCA: Results
DESCRIPTION OF THE SYSTEM BOUNDARY (X = INCLUDED IN LCA; ND = MODULE OR INDICATOR NOT
DECLARED; MNR = MODULE NOT RELEVANT)
BENEFITS AND
CONSTRUCTI LOADS
PRODUCT STAGE ON PROCESS USE STAGE END OF LIFE STAGE BEYOND THE
STAGE SYSTEM
BOUNDARIES
7 Environmental Product Declaration Hilti AG – HIT­HY 270
lairetam
waR
ylppus tropsnarT
gnirutcafunaM
eht
morf
tropsnarT
etis
eht
ot
etag
ylbmessA esU
ecnanetniaM
riapeR
tnemecalpeR tnemhsibrufeR
ygrene
lanoitarepO esu
retaw
lanoitarepO esu
noitcurtsnoc­eD
noitilomed tropsnarT
gnissecorp
etsaW
lasopsiD ­esueR ­yrevoceR ­gnilcyceR laitnetop
A1 A2 A3 A4 A5 B1 B2 B3 B4 B5 B6 B7 C1 C2 C3 C4 D
X X X X X ND ND MNR MNR MNR ND ND X X X X X
RESULTS OF THE LCA - ENVIRONMENTAL IMPACT according to EN 15804+A2: 1 kg HIT-HY 270
Core Indicator Unit A1 A2 A3 A4 A5 C1 C2 C3 C4 D
GWP­total [kg CO2­Eq.] 2.51E+0 4.87E­2 6.07E­1 7.12E­2 5.14E­1 4.02E­3 4.84E­3 0.00E+0 1.14E­1 0.00E+0
GWP­fossil [kg CO2­Eq.] 2.48E+0 4.86E­2 4.97E­1 7.09E­2 5.03E­1 4.02E­3 4.82E­3 0.00E+0 1.14E­1 0.00E+0
GWP­biogenic [kg CO2­Eq.] 2.71E­2 1.41E­4 1.09E­1 2.46E­4 1.07E­2 3.65E­6 1.67E­5 0.00E+0 2.85E­4 0.00E+0
GWP­luluc [kg CO2­Eq.] 1.45E­3 2.38E­5 9.37E­4 2.84E­5 2.62E­4 4.00E­7 1.93E­6 0.00E+0 2.15E­6 0.00E+0
ODP [kg CFC11­Eq.] 2.70E­7 1.09E­8 9.05E­8 1.64E­8 6.04E­8 8.59E­10 1.12E­9 0.00E+0 3.10E­9 0.00E+0
AP [mol H+­Eq.] 1.37E­2 3.66E­4 2.35E­3 2.02E­4 2.15E­3 4.17E­5 1.37E­5 0.00E+0 7.63E­5 0.00E+0
EP­freshwater [kg P­Eq.] 6.47E­4 3.06E­6 1.61E­4 4.85E­6 1.44E­4 1.27E­7 3.30E­7 0.00E+0 8.58E­7 0.00E+0
EP­marine [kg N­Eq.] 2.72E­3 8.00E­5 5.94E­4 4.11E­5 3.73E­4 1.85E­5 2.79E­6 0.00E+0 2.14E­3 0.00E+0
EP­terrestrial [mol N­Eq.] 2.21E­2 8.85E­4 4.83E­3 4.47E­4 5.08E­3 2.03E­4 3.03E­5 0.00E+0 3.07E­4 0.00E+0
POCP [kg NMVOC­Eq.] 8.79E­3 2.63E­4 1.51E­3 1.72E­4 1.09E­3 5.57E­5 1.17E­5 0.00E+0 1.12E­4 0.00E+0
ADPE [kg Sb­Eq.] 3.19E­5 1.59E­7 2.10E­6 2.56E­7 6.94E­6 2.04E­9 1.74E­8 0.00E+0 3.11E­8 0.00E+0
ADPF [MJ] 4.33E+1 7.02E­1 9.20E+0 1.06E+0 5.42E+0 5.41E­2 7.17E­2 0.00E+0 2.22E­1 0.00E+0
[m³ world­Eq
WDP 1.72E+0 3.15E­3 2.30E­1 4.94E­3 1.91E­1 1.45E­4 3.36E­4 0.00E+0 2.30E­3 0.00E+0
deprived]
GWP = Global warming potential; ODP = Depletion potential of the stratospheric ozone layer; AP = Acidification potential of land and water; EP =
Caption Eutrophication potential; POCP = Formation potential of tropospheric ozone photochemical oxidants; ADPE = Abiotic depletion potential for non­
fossil resources; ADPF = Abiotic depletion potential for fossil resources; WDP = Water (user) deprivation potential
RESULTS OF THE LCA - INDICATORS TO DESCRIBE RESOURCE USE according to EN 15804+A2: 1 kg
HIT-HY 270
Indicator Unit A1 A2 A3 A4 A5 C1 C2 C3 C4 D
PERE [MJ] 1.74E+0 9.50E­3 7.58E­1 1.54E­2 2.53E­1 3.09E­4 1.04E­3 0.00E+0 1.17E­2 0.00E+0
PERM [MJ] 0.00E+0 0.00E+0 5.63E­1 0.00E+0 3.94E­2 0.00E+0 0.00E+0 0.00E+0 0.00E+0 0.00E+0
PERT [MJ] 1.74E+0 9.50E­3 1.32E+0 1.54E­2 2.93E­1 3.09E­4 1.04E­3 0.00E+0 1.17E­2 0.00E+0
PENRE [MJ] 3.16E+1 7.03E­1 6.27E+0 1.06E+0 4.36E+0 5.41E­2 7.17E­2 0.00E+0 2.22E­1 0.00E+0
PENRM [MJ] 1.17E+1 0.00E+0 2.93E+0 0.00E+0 1.07E+0 0.00E+0 0.00E+0 0.00E+0 0.00E+0 0.00E+0
PENRT [MJ] 4.33E+1 7.03E­1 9.20E+0 1.06E+0 5.42E+0 5.41E­2 7.17E­2 0.00E+0 2.22E­1 0.00E+0
SM [kg] 8.78E­3 2.63E­4 6.91E­2 3.59E­4 7.10E­3 2.12E­5 2.44E­5 0.00E+0 8.41E­5 0.00E+0
RSF [MJ] 9.82E­5 2.38E­6 5.78E­3 3.96E­6 4.38E­4 6.91E­8 2.69E­7 0.00E+0 3.83E­6 0.00E+0
NRSF [MJ] 0.00E+0 0.00E+0 0.00E+0 0.00E+0 0.00E+0 0.00E+0 0.00E+0 0.00E+0 0.00E+0 0.00E+0
FW [m³] 4.31E­2 8.36E­5 5.63E­3 1.35E­4 4.72E­3 3.28E­6 9.14E­6 0.00E+0 2.92E­4 0.00E+0
PERE = Use of renewable primary energy excluding renewable primary energy resources used as raw materials; PERM = Use of
renewable primary energy resources used as raw materials; PERT = Total use of renewable primary energy resources; PENRE = Use of
non­renewable primary energy excluding non­renewable primary energy resources used as raw materials; PENRM = Use of non­
Caption
renewable primary energy resources used as raw materials; PENRT = Total use of non­renewable primary energy resources; SM = Use
of secondary material; RSF = Use of renewable secondary fuels; NRSF = Use of non­renewable secondary fuels; FW = Use of net fresh
water
RESULTS OF THE LCA – WASTE CATEGORIES AND OUTPUT FLOWS according to EN 15804+A2:
1 kg HIT-HY 270
Indicator Unit A1 A2 A3 A4 A5 C1 C2 C3 C4 D
HWD [kg] 1.84E­1 8.50E­4 5.20E­2 1.20E­3 1.69E­1 7.23E­5 8.16E­5 0.00E+0 3.46E­4 0.00E+0
NHWD [kg] 2.40E+0 1.34E­2 5.92E­1 2.13E­2 3.67E­1 5.08E­4 1.45E­3 0.00E+0 1.00E+0 0.00E+0
RWD [kg] 5.76E­5 4.85E­6 1.55E­5 7.27E­6 1.46E­5 3.81E­7 4.93E­7 0.00E+0 1.47E­6 0.00E+0
CRU [kg] 0.00E+0 0.00E+0 0.00E+0 0.00E+0 0.00E+0 0.00E+0 0.00E+0 0.00E+0 0.00E+0 0.00E+0
MFR [kg] 1.36E­4 1.71E­5 3.98E­2 3.31E­6 8.87E­2 7.20E­8 2.25E­7 0.00E+0 1.21E­6 0.00E+0
MER [kg] 3.69E­6 1.80E­8 5.66E­7 2.66E­8 4.17E­7 1.15E­9 1.81E­9 0.00E+0 5.85E­9 0.00E+0
EEE [MJ] 1.47E­2 1.44E­4 1.06E­2 2.30E­4 2.73E­3 2.12E­5 1.56E­5 0.00E+0 4.53E­4 0.00E+0
EET [MJ] 6.33E­2 6.78E­4 3.25E­2 9.56E­4 1.01E­2 2.15E­4 6.49E­5 0.00E+0 1.22E­3 0.00E+0
HWD = Hazardous waste disposed; NHWD = Non­hazardous waste disposed; RWD = Radioactive waste disposed; CRU = Components
Caption for re­use; MFR = Materials for recycling; MER = Materials for energy recovery; EEE = Exported electrical energy; EEE = Exported
thermal energy
RESULTS OF THE LCA – additional impact categories according to EN 15804+A2-optional:
1 kg HIT-HY 270
Indicator Unit A1 A2 A3 A4 A5 C1 C2 C3 C4 D
[Disease
PM 1.18E­7 3.48E­9 2.64E­8 5.72E­9 2.06E­8 1.12E­9 3.88E­10 0.00E+0 1.62E­9 0.00E+0
Incidence]
[kBq U235­
IRP 1.47E­1 3.62E­3 3.89E­2 5.54E­3 2.48E­2 2.48E­4 3.76E­4 0.00E+0 1.48E­3 0.00E+0
Eq.]
ETP­fw [CTUe] 8.24E+1 5.67E­1 7.85E+0 8.81E­1 1.46E+1 3.25E­2 5.98E­2 0.00E+0 4.83E­1 0.00E+0
HTP­c [CTUh] 7.40E­9 2.13E­11 3.11E­10 2.71E­11 7.60E­10 1.25E­12 1.84E­12 0.00E+0 7.12E­12 0.00E+0
HTP­nc [CTUh] 1.05E­7 5.32E­10 6.13E­9 8.63E­10 1.07E­8 2.35E­11 5.86E­11 0.00E+0 1.81E­10 0.00E+0
SQP [­] 5.08E+0 4.37E­1 4.08E+0 7.50E­1 1.15E+0 7.03E­3 5.09E­2 0.00E+0 5.83E­1 0.00E+0
PM = Potential incidence of disease due to PM emissions; IR = Potential Human exposure efficiency relative to U235; ETP­fw = Potential
Caption comparative Toxic Unit for ecosystems; HTP­c = Potential comparative Toxic Unit for humans (cancerogenic); HTP­nc = Potential
comparative Toxic Unit for humans (not cancerogenic); SQP = Potential soil quality index
Disclaimer 1 – for the indicator “Potential Human exposure efficiency relative to U235”.
This impact category deals mainly with the eventual impact of low dose ionizing
radiation on human health of the nuclear fuel cycle. It does not consider effects due to possible
nuclear accidents, occupational exposure nor due to radioactive waste disposal in underground
facilities. Potential ionizing radiation from the soil, from radon and from some construction materials is also not
measured by this indicator.
Disclaimer 2 – for the indicators “abiotic depletion potential for non­fossil resources”, “abiotic depletion potential
for fossil resources”, “water (user) deprivation potential, deprivation­weighted water consumption”, “potential
comparative toxic unit for ecosystems”, “potential comparative toxic unit for humans – cancerogenic”, “Potential
comparative toxic unit for humans ­ not cancerogenic”, “potential soil quality index”.
The results of this environmental impact indicator shall be used with care as the
uncertainties on these results are high or as there is limited experienced with the indicator.
6. LCA: Interpretation
The dominance analysis shows that the main causes
of environmental impacts and indicators can be found In the information module A1, the material supply of
in the information module A1. This shows the global the reaction resin mixture causes more than 80% of
warming potential for the provision of material with the global warming potential.
about 65%, based on all information modules. Modules
A4 and A5 also represent an import part of the final
impact.
Illustration: Dominance analysis A1
The mass of the individual components of the resin
mixture come from the recipe information provided by
Illustration: Dominance analysis A1- C4 the manufacturer. According to the manufacturer, this
information can be assumed to be highly accurate.
Module A1 is detailed below. Module A3’s global The relevant datasets used to calculate the material
warming impact is mostly constituted by the final availability of the product are highly topical since the
product packaging (11% of the total impact) and raw materials were detailed as much as necessary to
energy for manufacturing (3% of the total impact). Most find corresponding data in the latest Ecoinvent
of the global warming impact from module A5 is database (2021). The locations were also respected.
caused by the product losses (6% of the final impact) Since these datasets strongly influence the results, as
the end­of­life of the soiled product packaging, treated shown by the dominance analysis, so does the overall
as hazardous waste (4% of the final impact). computation.
7. Requisite evidence
Hilti HIT­HY 270 complies with the requirements of  emission class A+ outlined in the French VOC
 DIBt (2010) in combination with the NIK Directives (2020) in accordance with the
values from AgBB (2018) for applications in Eurofins attestation,
interior areas,  CDPH/EHLB Standard Method V 1.2 (2017)
8 Environmental Product Declaration Hilti AG – HIT­HY 270
in accordance with Eurofins test report, No. 392­2020­ R (dimensionless) <1 ­
00549101_A_EN, Eurofins test report, No. 392­2020­ VOC without NIK <100 μg/m3
00549101_A_EN and Eurofins test report, No. 392­ Carcinogenic Substances <1 μg/m3
2020­00549101_H_EN respectively.
AgBB overview of results (3 days [µg/m³])
Name Value Unit
AgBB overview of results (28 days [µg/m³]) VOC without NIK <10000 μg/m3
Name Value Unit Carcinogenic Substances <10 μg/m3
TVOC (C6 ­ C16) <1000 μg/m3
Sum SVOC (C16 ­ C22) <100 μg/m3
8. References
Standards Category Rules for Construction Products from the
range of Environmental Product Declarations for
DIN EN 13501-1 Institut Bauen und Umwelt (IBU), Part A: Calculation
Klassifizierung von Bauprodukten und Bauarten zu Rules for the Life Cycle Assessment and
ihrem Brandverhalten Requirements on the Project Report according to EN
15804+A2:2019, 2021­04
DIN EN 14293 PCR Part B
Klebstoffe ­ Klebstoffe für das Kleben von Parkett auf Institut Bauen und Umwelt e.V, Berlin (pub.): Product
einen Untergrund ­ Prüfverfahren und Category Rules for Construction Products from the
Mindestanforderungen range of Environmental Product Declarations for
Institut Bauen und Umwelt (IBU), Part B: Requirements
on the EPD for Reaction resin products, 2019­01
DIN EN ISO 50001
DIN EN ISO 50001: 2018 Energy management
systems ­ Requirements with guidance for use
Further References
EN 15804
EN 15804:2012+A1:2013, Sustainability of AFNOR, «FD P01-015» 2006
construction works — Environmental Product Qualité environnementale des produits de construction
Declarations — Core rules for the product category of ­ Fascicule de données énergie et transport
construction products.
AgBB (2018)
EN 15804 Vorgehensweise bei der gesundheitlichen Bewertung
EN 15804:2012+A2:2019, Sustainability of der Emissionen von flüchtigen organischen
construction works — Environmental Product Verbindungen (VVOC, VOC und SVOC) aus
Declarations — Core rules for the product category of Bauprodukten (2018)
construction products.
Candidate List of substances of very high concern
EN ISO 604 for Authorisation
DIN EN ISO 604:2003­12: Determination of European Cheminals Agency (ECHA), in accordance
compressive properties with Article 50(10) of the REACH regulation
CDPH/EHLB/Standard Method V1.2
EN ISO 1183-1 California CDPH Standard Method is a US standard for
DIN 51757:2011­01 Plastics ­ Methods for determining evaluating and restricting VOC emissions to indoor air.
the density of non­cellular plastics ­ Part 1: Immersion Developed in California as "Section 01350"
method, liquid pyknometer method and titration Specification, several systems in the US refer to CDPH
method Standard Method
Comité National Routier (CNR)
ISO 9001 Enquête longue distance, PARIS, 2019
ISO 9001:2015 Quality management systems ­
Requirements DIBt (2010)
Grundsätze zur gesundheitlichen Bewertung von
Bauprodukten in Innenräumen (Oktober 2010)
ISO 14001 Eurofins test report, No. 392­2019­00435401_D_EN
ISO 14001:2015 Environmental management systems VOC test report for verification of compliance with
­ Requirements with guidance for use DIBt(2010)/AgBB(2018)
ISO 14025 Eurofins test report, No. 392-2020-00549101_A_EN
EN ISO 14025:2011, Environmental labels and VOC test report for verification of compliance with
declarations — Type III environmental declarations — DIBt(2010)/AgBB(2018)
Principles and procedures.
Eurofins test report, No. 392-2020-00549101_A_EN
PCR Part A VOC test report for verification of compliance with the
Institut Bauen und Umwelt e.V, Berlin (pub.): Product French VOC directive from 2020
9 Environmental Product Declaration Hilti AG – HIT­HY 270
Umwelt Bundesamt: Herkunftsnachweisregister
Eurofins test report, 392-2020-00549101_H_EN (HKNR) — Entwertungsnachweis durch GETECH
VOC test report for verification of compliance with ENERGIE GMBH für HILTI
CDPH/EHLB/Standard Method V1.2 from 2017
European Waste code
in accordance with the European Waste Catalogue Database
(EWC) (EWC 2014/955/EU) Commission Decision
amending Decision 2000/532/EC on the list of waste Ecoinvent 3.8
pursuant to Directive 2008/98/EC of the European ecoinvent Version 3
Parliament and of the Council Wernet, G., Bauer, C., Steubing, B., Reinhard, J.,
Moreno­Ruiz, E., and Weidema, B., 2016. The
ETA 13/1036 ecoinvent database version 3 (part I): overview and
European Technical Approval Hilti HIT­HY 270 methodology. The International Journal of Life Cycle
Assessment, [online] 21(9), pp.1218–1230. Available
ETA 19/0160 at: <http://link.springer.com/10.1007/s11367­016­1087­
European Technical Approval Hilti HIT­HY 270 8> [Accessed in 2021/2022].
French VOC Directives
Décret no 2011­321 du 23 mars 2011 relatif à
l’étiquetage des produits de construction ou de Publication
revêtement de mur ou de sol et des peintures et vernis
sur leurs émissions de polluants volatils IBU 2021
Arrêté du 19 avril 2011 relatif à l’étiquetage des Institut Bauen und Umwelt e.V.: General Instructions
produits de construction ou de revêtement de mur ou for the EPD programme of Institut Bauen und Umwelt
de sol et des peintures et vernis sur leurs émissions de e.V., Version 2.0, Berlin: Institut Bauen und Umwelt
polluants volatils e.V., 2021
www.ibu­epd.com
NSF
NSF/ANSI/CAN 61 Drinking Water System
Components ­ Health Effects
Umwelt Bundesamt 2021
10 Environmental Product Declaration Hilti AG – HIT­HY 270
Publisher
Institut Bauen und Umwelt e.V. Tel +49 (0)30 3087748­ 0
Hegelplatz 1 Fax +49 (0)30 3087748­ 29
10117 Berlin Mail info@ibu­epd.com
Germany Web www.ibu-epd.com
Programme holder
Institut Bauen und Umwelt e.V. Tel +49 (0)30 ­ 3087748­ 0
Hegelplatz 1 Fax +49 (0)30 – 3087748 ­ 29
10117 Berlin Mail info@ibu­epd.com
Germany Web www.ibu-epd.com
Author of the Life Cycle
Assessment Tel +33 (0)9 53 23 98 30
ESTEANA Fax ­
Rue Mège 26 Mail contact@esteana.fr
83220 Le Pradet Web www.esteana.fr
France
Owner of the Declaration
Hilti Aktiengesellschaft Tel +423 234 2111
Feldkircher Strasse 100 Fax +423 234 2965
9494 Schaan Mail HAGHSE@hilti.com
Liechtenstein Web www.hilti.com
