ENVIRONMENTAL PRODUCT DECLARATION
as per ISO 14025 and EN 15804+A1
Owner of the Declaration ArcelorMittal Construction
Programme holder Institut Bauen und Umwelt e.V. (IBU)
Publisher Institut Bauen und Umwelt e.V. (IBU)
Declaration number EPD-AMC-20210146-CBB3-EN
Issue date 23.06.2022
Valid to 30.01.2027
Building Steel Profiles
ArcelorMittal Construction
www.ibu-epd.com | https://epd-online.com
Umwelt Produktdeklaration Name des Herstellers – Name des Produkts
General Information
ArcelorMittal Construction Building Steel Profiles
Programme holder Owner of the declaration
IBU – Institut Bauen und Umwelt e.V. ArcelorMittal Construction
Hegelplatz 1 Morinval
10117 Berlin 55800 Contrisson
Germany France
Declaration number Declared product / declared unit
EPD-AMC-20210146-CBB3-EN The declared unit is 1m² of galvanized or organic
coated steel profile from the ArcelorMittal Construction
product range.
This declaration is based on the product Scope:
category rules: The Life Cycle Assessment is based on data collected
Thin walled profiles and profiled panels of metal, 01.2019 from the ArcelorMittal plants producing galvanized or
(PCR checked and approved by the SVR) organic coated steel profiles, representing 95% of the
production in 2019.
Issue date
23.06.2022 The owner of the declaration shall be liable for the
underlying information and evidence; the IBU shall not
be liable with respect to manufacturer information, life
Valid to
cycle assessment data and evidences.
30.01.2027
The EPD was created according to the specifications
of EN 15804+A1. In the following, the standard will be
simplified as EN 15804.
Verification
The standard EN 15804 serves as the core PCR
Independent verification of the declaration and data
according to ISO 14025:2011
Dipl. Ing. Hans Peters internally x externally
(chairman of Institut Bauen und Umwelt e.V.)
Dr. Alexander Röder Matthias Klingler
(Managing Director Institut Bauen und Umwelt e.V.)) (Independent verifier)
Product
Product description/Product definition They are produced in the ArcelorMittal Construction
This Environmental Product Declaration refers to production plants located in Austria (Neuhofen),
galvanized or organic coated steel profile produced by Belgium (Geel), France (Cérons, Diémoz, Haironville,
ArcelorMittal Construction. These products are made La Magdeleine, Montataire, Nérac, Strasbourg,
of cold-rolled steel profiles for roof, wall, facades and Thouaré and Contrisson), Germany (Brehna and
floors applications. Reichshof), The Netherlands (Tiel), Poland (Rawa,
Swietochlowice and Starachowice), Portugal (Cartaxo),
The targeted applications are as follow: Romania (Pantelimon), Slovakia (Senika), Spain
 Roof & Decking (Berrioplano and Cervera) and Sweden (Sveg and
 Traditional wall Karlstad).
 Facade architectural
For the placing on the market of the product in the
 Sidings
European Union/European Free Trade Association
 Cassettes (EU/EFTA) (with the exception of Switzerland)
 Wall liner trays Regulation (EU) No. 305/2011 (CPR) applies. The
product needs a declaration of performance and the
 Floors
CE-marking taking into consideration one of the
following standards:
These profiles are available in different thicknesses  EN 1090-1:2009 Execution of steel and
from 0.4 to 1.5 mm. They can be covered with different
aluminium structures – Part 1: Procedures for
metallic coating with masses from 60 to 350 g/m².
attestation of conformity for load-bearing
They also can be constituted of an organic coating with
components and the CE-marking;
thicknesses from 12 to 205 µm, applied on the metallic
coating.  EN 14782:2006 Self-supporting metal sheet
for roofing, external cladding and internal
2 Environmental Product Declaration ArcelorMittal – Building Steel Profiles
lining - Product specification and sheet and strip for roofing, external cladding and
requirements and internal lining - Product specification and requirements.
 EN 14783:2013 Fully supported metal sheet
Base materials/Ancillary materials
and strip for roofing, external cladding and
The products covered by this Environmental Product
internal lining - Product specification and
Declaration are steel profiles produced in the different
requirements. production plants of ArcelorMittal Construction. They
are mainly composed of a galvanized and pre-painted
steel sheet with organic coating in some cases.
For the application and use the respective national
Steel is mainly iron and carbon, with small amounts of
provisions apply.
alloying elements. These elements modify the
chemical and physical properties of steel such as
Application
strength, durability and corrosion resistance. High
Steel profiles, covered by this EPD, are used as roof,
strength low alloyed (HSLA) carbon steel has a carbon
wall, façade and floors for all types of construction.
content lower than 0.2 %.
The wide range of profiles meets the different
The metallic coating includes only Zinc or Zinc,
performance needs: structural, acoustic, thermal, fire
Aluminum and Magnesium. The organic coatings are
resistance.
made from polyester, polyurethane or polyvinylidene
fluoride (PVDF) resins.
Technical Data
The final product (i.e. metallic layer plus organic,
This product contains substances listed in the
where applied, coating and forming shape) varies
candidate list (date: 02.05.2021) exceeding 0.1
according to the intended end use of the products.
percentage by mass: no.
Reference service life
Constructional data
The reference service life for the profile product range
is not declared, since the lifetime will depend on
Performance data of the product in accordance with
specific applications as well as environmental
the declaration of performance with respect to its
conditions.
essential characteristics according to EN 1090-1:2009
Execution of steel and aluminium structures – Part 1:
As a structural part of the building, steel profiles are
Procedures for attestation of conformity for load-
expected and specified to reach the same service life
bearing components or EN 14782:2006 Self-
as that of the building. The steel reference service life
supporting metal sheet for roofing, external cladding
can be up to 100 years.
and internal lining - Product specification and
requirements or EN 14783:2013 Fully supported metal
LCA: Calculation rules
Declared Unit  Transport of resources and additives to the
The declared unit is 1 m² of metallic or metallic and production site. Production processes on-site
organic coated steel profile in the ArcelorMittal
including energy, production of additives,
Construction product range.
disposal of production residues, and
consideration of related emissions
Declared unit
Name Value Unit  Recycling of production/manufacturing scrap.
Declared unit 1 m2 Steel scrap is assumed to reach the end-of-
conversion factor [Mass/Declared waste status once it is shredded and sorted,
6.16 -
Unit] (surface weight in kg/m²) thus becoming the input to the product
system in the inventory.
The mean product described in this EPD has been
determined to give an average value for the most
representative product in terms of volume production. Module C3 takes into account the sorting and
The use of this mean value allows extrapolation on the shredding of after-use steel that is recycled, as well as
global range with a relative difference on global the non-recovered scrap due to sorting efficiency
warming potential not exceeding 9 % of the extreme which is landfilled. A conservative value of 2 % landfill
thickness. is considered.
Module D refers to the end-of-life of metallic or
System boundary metallic and organic coated steel profile, including
Type of the EPD: cradle-to-gate - with options. Module reuse and recycling. For recycling, the net amount of
A1-A3, Module C3 and module D were considered. steel scrap made available over the whole life cycle is
considered.
Modules A1-A3 of metallic or metallic and organic
coated steel profile production include the following: Comparability
 The provision of resources, additives, and Basically, a comparison or an evaluation of EPD data
is only possible if all the data sets to be compared
energy
3 Environmental Product Declaration ArcelorMittal – Building Steel Profiles
were created according to EN 15804 and the building Gabi Envision version 9.2.1.68, based on SP35,
context, respectively the product-specific created with GaBi ts Software version 8.7 was used to
characteristics of performance, are taken into account. calculate this EPD.
LCA: Scenarios and additional technical information
The end of life for average metallic or metallic and
organic coated steel profile products consists of 98 %
recycling and 2 % landfill, with the corresponding
benefits and burdens. This is based on the European
Commission Technical Steel Research, the German
Ministry of Environmental Affairs and internal
documentation within ArcelorMittal.
End of life (C1-C4)
Name Value Unit
Recycling 6.032 kg
Landfilling 0.123 kg
Reuse, recovery and/or recycling potentials (D),
relevant scenario information
Name Value Unit
Recycling 98 %
4 Environmental Product Declaration ArcelorMittal – Building Steel Profiles
LCA: Results
DESCRIPTION OF THE SYSTEM BOUNDARY (X = INCLUDED IN LCA; MND = MODULE NOT DECLARED;
MNR = MODULE NOT RELEVANT)
BENEFITS AND
CONSTRUCTI LOADS
PRODUCT STAGE ON PROCESS USE STAGE END OF LIFE STAGE BEYOND THE
STAGE SYSTEM
BOUNDARIES
5 Environmental Product Declaration ArcelorMittal – Building Steel Profiles
lairetam
waR
ylppus tropsnarT
gnirutcafunaM
eht
morf
tropsnarT
etis
eht
ot
etag
ylbmessA esU
ecnanetniaM
riapeR
tnemecalpeR tnemhsibrufeR
ygrene
lanoitarepO esu
retaw
lanoitarepO esu
noitcurtsnoc-eD
noitilomed tropsnarT
gnissecorp
etsaW
lasopsiD -esueR -yrevoceR -gnilcyceR laitnetop
A1 A2 A3 A4 A5 B1 B2 B3 B4 B5 B6 B7 C1 C2 C3 C4 D
X X X MND MND MND MND MNR MNR MNR MND MND MND MND X MND X
RESULTS OF THE LCA - ENVIRONMENTAL IMPACT according to EN 15804+A1: 1 m² Building Steel
Profiles
Parameter Unit A1-A3 C3 D
Global warming potential [kg CO2-Eq.] 1.80E+1 1.23E-2 -1.09E+1
Depletion potential of the stratospheric ozone layer [kg CFC11-Eq.] 3.60E-11 4.24E-14 2.15E-12
Acidification potential of land and water [kg SO2-Eq.] 3.41E-2 4.17E-5 -2.63E-2
Eutrophication potential [kg (PO4)3--Eq.] 3.31E-3 4.92E-6 -2.25E-3
Formation potential of tropospheric ozone photochemical
[kg ethene-Eq.] 5.68E-3 2.93E-6 -3.38E-3
oxidants
Abiotic depletion potential for non-fossil resources [kg Sb-Eq.] 6.53E-4 5.86E-9 1.12E-6
Abiotic depletion potential for fossil resources [MJ] 1.72E+2 1.38E-1 -8.65E+1
RESULTS OF THE LCA - INDICATORS TO DESCRIBE RESOURCE USE according to EN 15804+A1: 1 m²
Building Steel Profiles
Parameter Unit A1-A3 C3 D
Renewable primary energy as energy carrier [MJ] 1.42E+1 6.89E-2 7.92E+0
Renewable primary energy resources as material utilization [MJ] 0.00E+0 0.00E+0 0.00E+0
Total use of renewable primary energy resources [MJ] 1.42E+1 6.89E-2 7.92E+0
Non-renewable primary energy as energy carrier [MJ] 1.82E+2 2.11E-1 -8.16E+1
Non-renewable primary energy as material utilization [MJ] 0.00E+0 0.00E+0 0.00E+0
Total use of non-renewable primary energy resources [MJ] 1.82E+2 2.11E-1 -8.16E+1
Use of secondary material [kg] 2.99E-1 0.00E+0 5.73E+0
Use of renewable secondary fuels [MJ] 0.00E+0 0.00E+0 0.00E+0
Use of non-renewable secondary fuels [MJ] 0.00E+0 0.00E+0 0.00E+0
Use of net fresh water [m³] 4.69E-2 9.43E-5 3.83E-3
RESULTS OF THE LCA – WASTE CATEGORIES AND OUTPUT FLOWS according to EN 15804+A1:
1 m² Building Steel Profiles
Parameter Unit A1-A3 C3 D
Hazardous waste disposed [kg] 3.61E-7 1.34E-9 -5.73E-8
Non-hazardous waste disposed [kg] 1.14E-1 1.23E-1 -1.74E-1
Radioactive waste disposed [kg] 3.91E-3 2.89E-5 1.95E-3
Components for re-use [kg] 0.00E+0 0.00E+0 0.00E+0
Materials for recycling [kg] 0.00E+0 6.03E+0 0.00E+0
Materials for energy recovery [kg] 0.00E+0 0.00E+0 0.00E+0
Exported electrical energy [MJ] 0.00E+0 0.00E+0 0.00E+0
Exported thermal energy [MJ] 0.00E+0 0.00E+0 0.00E+0
Note: 0.29912 kg scrap is used to manufacture 6.1555 kg of 1 m² of Building Steel Profiles. After use, 6.0324 kg
steel is recycled, 0 kg is reused. The potential environmental impact calculated for module D depends on the net
amount of scrap left in the system, which is 6.0324 - 0.29912 - 0 = 5.7333 kg . This means that the system
produces a net steel scrap output of 5.7333 kg, thus module D shows an environmental benefit.
References
EN 1090 Declarations — Core rules for the product category of
EN 1090-1:2009 Execution of steel and aluminium construction products.
structures – Part 1: Procedures for attestation of
conformity for load-bearing components. EN 14782
EN 14782:2006 Self-supporting metal sheet for
EN 15804 roofing, external cladding and internal lining - Product
EN 15804:2012+A1:2013 - Sustainability of specification and requirements.
construction works — Environmental Product
EN 14783 PCR - Part A: Calculation Rules for the Life Cycle
EN 14783:2013 Fully supported metal sheet and strip Assessment and Requirements on the Project Report,
for roofing, external cladding and internal lining - Institut Bauen und Umwelt e.V., www.bauumwelt.com,
Product specification and requirements. 2019.
ISO 14025 PCR Part B
DIN EN ISO 14025:2011-10 - Environmental labels PCR - Part B: Requirements of the EPD for Thin
and declarations — Type III environmental walled profiles and profiled panels of metal, Institut
declarations — Principles and procedures. Bauen und Umwelt e.V., www.bauumwelt.com, 2019.
European Commission Technical Steel Research Candidate list - REACH
Sansom, M.and Meijer, J.:Life-cycle assessment (LCA) Regulation (EC) No 1907/2006 of the European
for steel construction, European Commission technical Parliament and of the Council on the Registration,
steel research, 2001-12. Evaluation, Authorisation and Restriction
of Chemicals (REACH)
GaBi Envision https://echa.europa.eu/candidate-list-table
GaBi Software System and Database for Life Cycle
Engineering, thinkstep AG, Leinfelden-Echterdingen, ArcelorMittal EPD I-tool
2019 (http://documentation.gabi-software.com/). I-tool for EPD developed by thinkstep AG 17.12.2018.
File: 2021_05_17_iTool_Profiles.
GaBi ts Software
GaBi ts dataset documentation for the GaBi Software CPR
System and Database for Life Cycle Engineering, Regulation (EU) No 305/2011 of the European
thinkstep AG, Leinfelden-Echterdingen, 2019 parliament and of the council of 9 March 2011 laying
(http://documentation.gabi-software.com/). down harmonised conditions for the marketing of
construction products and repealing Council Directive
IBU 2021 89/106/EEC.
General Instructions for the EPD programme of Institut
Bauen und Umwelt e.V. Version 2.0, Berlin: Institut
Bauen und Umwelt e.V., 2021. www.ibu-epd.com
PCR Part A
6 Environmental Product Declaration ArcelorMittal – Building Steel Profiles
Publisher
Institut Bauen und Umwelt e.V. Tel +49 (0)30 3087748- 0
Hegelplatz 1 Fax +49 (0)30 3087748- 29
10117 Berlin Mail info@ibu-epd.com
Germany Web www.ibu-epd.com
Programme holder
Institut Bauen und Umwelt e.V. Tel +49 (0)30 - 3087748- 0
Hegelplatz 1 Fax +49 (0)30 – 3087748 - 29
10117 Berlin Mail info@ibu-epd.com
Germany Web www.ibu-epd.com
Author of the Life Cycle
Assessment Tel +33 3 29 70 75 03
ArcelorMittal Construction Fax -
Morinval - Mail
55800 Contrisson amcfcommercial@arcelormittal.c
France om
Web construction.arcelormittal.com
Owner of the Declaration
ArcelorMittal Construction Tel +33 3 29 70 75 03
Morinval - Fax -
55800 Contrisson Mail
France sustainability.amc@arcelormittal.
com
Web construction.arcelormittal.com
