ENVIRONMENTAL PRODUCT DECLARATION
as per ISO 14025 and EN 15804+A2
Owner of the Declaration Astron Buildings S.A
Publisher Institut Bauen und Umwelt e.V. (IBU)
Programme holder Institut Bauen und Umwelt e.V. (IBU)
Declaration number EPD-AST-20240035-IBI1-EN
Issue date 02.07.2024
Valid to 01.07.2029
Astron PRS Product (galvanized steel elements made of welded
sections)
Astron Buildings S.A.
www.ibu-epd.com | https://epd-online.com
1. General Information
Astron Buildings S.A. Astron PRS Product (galvanized steel elements
made of welded sections)
Programme holder Owner of the declaration
IBU – Institut Bauen und Umwelt e.V. Astron Buildings S.A
Hegelplatz 1 Route d’Ettelbruck 34
10117 Berlin 9230 Diekirch
Germany Luxembourg
Declaration number Declared product / declared unit
EPD-AST-20240035-IBI1-EN 1 t of PRS galvanized structural steel
This declaration is based on the product category rules: Scope:
Structural steels, 01.08.2021 The EPD represents 100% of galvanized PRS structural steel (steel
(PCR checked and approved by the SVR) elements made of welded sections) produced by Astron Building S.A. in
Diekirch.
The owner of the declaration shall be liable for the underlying information
Issue date and evidence; the IBU shall not be liable with respect to manufacturer
information, life cycle assessment data and evidences.
02.07.2024
The EPD was created according to the specifications of EN 15804+A2. In
the following, the standard will be simplified as EN 15804.
Valid to
01.07.2029 Verification
The standard EN 15804 serves as the core PCR
Independent verification of the declaration and data according to ISO
14025:2011
internally X externally
Dipl.-Ing. Hans Peters
(Chairman of Institut Bauen und Umwelt e.V.)
Florian Pronold Dr Naeem Adibi,
(Managing Director Institut Bauen und Umwelt e.V.) (Independent verifier)
1 Environmental Product Declaration - Astron Buildings S.A. - Astron PRS Product (galvanized steel elements made of welded sections)
2. Product
2.1 Product description/Product definition 2.5 Base materials/Ancillary materials
This EPD applies to 1 t of PRS structural steel. PRS are Structural steels are non-or low-alloy steel products whose
structural steel elements which are made up by cutting and carbon content is between 0 and 0.6 %. Iron is the main
welding steel plates to form structural sections including component of steel sections and plates. The content of other
gussets, stiffeners and connection plates. The Astron PRS steel alloy elements is significantly less. The exact chemical
elements are of the steel grade S355. composition is defined for the S355 steel grade in the EN
For the placing on the market of the product in the European 10025. The surfaces of hot-dip galvanized PRS elements are
Union/European Free Trade Association (EU/EFTA) (with the covered by a zinc coating.
exception of Switzerland) Regulation (EU) No. 305/2011 (CPR)
applies. The PRS elements need a declaration of performance Auxiliary materials:
(DoP) taking into consideration EN 1090-1, Execution of steel A. welding wire and welding sticks
and aluminium structures Part 1: Requirements for conformity B. welding powder or welding protection gas argon
assessment of structural components and the CE-marking. C. shot blast material SA2.5
Alternatively, the DoP and CE marking are based on the ETA- D. possibly corrosion protection paint in case of organic coating
18/1027 'Astron Building System". E. Degreasing agent, hydrochloric acid, zinc and ammonium
chloride, zinc alloy
For the application and use the respective national provisions
apply. 1) This product/article/at least one partial article contains
substances listed in the ECHA candidate list (date: 02.03.2022)
2.2 Application exceeding 0.1 percentage by mass:
Structural steel PRS elements are intended for bolted
• no
structures of industrial or other non-residential buildings, or in
2) This product/article/at least one partial article contains other
composite steel and concrete structures. Examples are:
carcinogenic, mutagenic, or toxic for reproduction (CMR)
• single-storey buildings (industrial fabrication and/or substances in categories 1A or 1B which are not on the ECHA
storage halls, exhibition halls, etc.) candidate list, exceeding 0.1 percentage by mass:
• multi-storey buildings (offices, shops, schools, car parks,
• no
etc.)
3) Biocide products were added to this construction product or it
• other industrial structures (power plants, sports or
has been treated with biocide products (this then concerns a
leisure centers, convention centers, stations, etc.)
treated product as defined by the (EU) Regulation on Biocidal
2.3 Technical Data Products No. 528/2012):
This EPD is valid for PRS steel elements of varied dimensions • no
and different forms of delivery. Specific information on
dimension tolerances, constructional data as well as 2.6 Manufacture
mechanical and chemical properties of the used steel can be The manufacturing follows the rules in EN 1090-2 Execution of
found in the relevant literature and/or the standards. steel structures and aluminium structures - Part 2: Technical
requirements for steel structures.
Hot-dip galvanizing (HDG) of PRS is performed according to
EN ISO 1461 and DASt Guideline 022 In the integrated PRS production line, the following steps are
executed:
Technical data of processed steel
• cutting of all sub-plates by shearing or plasma punching
Name Value Unit
/ drilling of holes
Density acc. EN 10025-1 7850 kg/m3
pre-assembling of web and flange
Modulus of elasticity 210000 N/mm2 • welding of the web flange under powder
Coefficient of thermal expansion acc. EN • final assembling of the complete element with tack
10025-1
12 10-6K-1
welding
• final welding of the PRS (manual or by robot)
Thermal conductivity acc. EN 10025-1 48 W/(mK)
Quality control: ISO 9001 monitoring according to the relevant
Melting point acc. EN 10025-1 1536 °C
product standards, e.g. EN 1090 and ETA18-1027, including
Shear modulus acc. EN 10025-1 81 kN/mm² FPC auditing by a third party.
Performance data of the product in accordance with the
declaration of performance with respect to its essential Subsequently, the PRS elements are hot-dip galvanized. For
characteristics according to: this purpose, they undergo a wet chemical surface cleaning,
are covered by flux, dried and then dipped in a hot zinc bath
• EN 1090-1, Execution of steel and aluminium structures
and cooled.
Part 1: Requirements for conformity assessment of
Quality assurance: ISO 9001 monitoring according to DASt
structural components
Guideline 022.
• ETA-18/1027 'Astron Building System
• EN ISO 1461, Hot dip galvanized coatings on fabricated 2.7 Environment and health during manufacturing
iron and steel articles - Specifications and test methods
No measures relating to safety, health and environmental
protection during the manufacturing process extending beyond
2.4 Delivery status
national guidelines are required.
The dimensions of the declared products may vary according to
the intended application. The surface condition may be 2.8 Product processing/Installation
untreated ('black'), painted or hot-dip galvanized (HDG).
Manufacturing/Erection:
Planning, manufacturing, erection and intended use of PRS
2 Environmental Product Declaration - Astron Buildings S.A. - Astron PRS Product (galvanized steel elements made of welded sections)
elements have to be carried out depending on the respective
applications according to the generally recognized rules of Hot-dip galvanizing allows for durable corrosion protection of
engineering and Astron erection recommendations. PRS steel components under atmospheric corrosion conditions.
The standards of EN 1993 and EN 1994 apply to the design of The protection normally lasts for several decades without any
steel structures and composite steel and concrete structures. need for maintenance or repair.
They include the requirements regarding serviceability, bearing Hot-dip galvanizing also provides adequate protection under
capacity, durability and fire resistance of steel structures (EC3) maritime conditions and against deicing salts. For more
and composite steel and concrete structures (EC4). information regarding the reference service life of hot-dip
The standards EN 1090, parts 1+2, or alternatively the ETA- galvanized structural steel, see ISO 14713-1.
18/1027 apply to the execution of structures made of PRS steel
elements and include the requirements for factory production
control. In addition, the European Standards will work in
connection with national amendments, national instructions,
guidelines and publications, as well as legal provisions.
Regarding transport and storage of PRS elements, the
generally accepted requirements for securing loads have to be
observed.
Occupational safety/Environmental protection:
When manufacturing/use PRS steel elements pursuant to the
generally recognized rules of engineering there are no
measures to be taken which are going beyond the public
occupational health and safety.
The manufacturing/using of the raw, i.e. unprotected PRS steel
elements, pursuant to the generally recognized rules of
engineering does not release substantial environmental 2.13 Extraordinary effects
pollutants. Particular measures to protect the environment are Fire
not required. The material is class A1, i.e. not flammable per EN 13501.
The plasma cutting, welding, painting and hot dip galvanization
Fire protection
activities must respect the respective national regulations for
Name Value
health and safety.
Building material class A1
Residual material: The material does not emit fumes or fire gases. The eventual
During processing residual pieces as well as turnings are to be paint layer is negligible in this matter.
separately collected. This scrap steel is entirely recycled by
melting and producing new steel products. Given the significantly lower emissivity of hot-dip galvanized
The recovered zinc can be used again for hot-dip galvanizing. structural steel, and depending on the form factor, fire
resistance class R30 can be achieved by hot-dip galvanizing
2.9 Packaging
alone and without any additional protective measures. At
Structural PRS elements are delivered unpacked. To facilitate
temperatures above 650°C, the thin zinc coating evaporates
loading/unloading and protect during transportation, the
quickly as zinc oxide (ZnO), causing fumes. When inhaled for a
material is generally stacked with wooden battens in between
prolonged period of time, ZnO fumes can cause metal fume
them. For sea transport, special packaging to protect the goods
fever (diarrhoea, fever, dry throat), whereby these symptoms
while at sea might be used.
normally disappear within 1 to 2 days after inhalation. The
critical temperature (failure temperature of the component)
2.10 Condition of use
depends primarily on the component load and the fire insulation
PRS elements are made from steel grades which are non- /low-
of the component.
alloyed steel products generated by alloying iron with other
metals and nonmetals (esp. carbon). Iron is the main
component of steel sections and plates. The components are
Water
listed under chapter 2.5 'Base materials'. During usage, no
Steel is stable in water, insoluble and does not emit substances
changes in material composition shall occur.
in water. In case of flooding no impacts are to be expected.
Steel can corrode in the presence of oxygen in the water (=
Hot-dip galvanized PRS elements have a zinc layer, which
slow oxidation).
thickness is normalized in EN ISO 1461. Colour-coated PRS
Hot-dip galvanized steel is not soluble in water and does not
elements have an organic paint layer for corrosion protection.
release any substances when exposed to water.
2.11 Environment and health during use
Mechanical destruction
The intended use of PRS elements does not hazard health or
Due to the ductility of steel, PRS steel structures react
the environment in any known way. If used properly, there are
resiliently in the event of unforeseeable mechanical destruction:
no known negative impacts of hot dip galvanized PRS sections
In case of tensile load necking will occur before cracking. In
on the environment or on the health of people.
case of a lasting high compression load, components of steel
2.12 Reference service life may buckle or bulge. No splintering or breaking edges shall
In general, the reference service life is not relevant for result.
consideration of the LCA. As construction products with many
2.14 Re-use phase
different applications, a reference service life for structural PRS
General:
steel elements is not declared here. The purpose, possible
PRS steel elements are recyclable by 100 %. Due to the
corrosion protection and adequate maintenance are decisive
magnetic properties of steel, >99 % of the used steel is
for service life.
regained after dismantling (European Commission Technical
3 Environmental Product Declaration - Astron Buildings S.A. - Astron PRS Product (galvanized steel elements made of welded sections)
Steel Research). recycling. However, in case of dumping due to collection loss
no environmental impacts are expected.
Re-use
PRS steel elements can be re-used. Currently, around 11 % of Waste code according to European Waste Catalogue: 17 04 05
the products are re-used after dismantling. - iron and steel
Recycling: 2.16 Further information
PRS steel elements can be recycled without any problems after Additional information on constructing with PRS and with steel
dismantling. Currently, around 88 % of the products are used in general can be obtained from many public sources, for
for closed-loop recycling (including 1 % loss). Data from example:
industry estimates based on the following sources: European • Astron.biz
Commission Technical Steel Research and Bundesministerium • bauforumstahl.de
für Umwelt, Naturschutz, Bau und Reaktorsicherheit. • cticm.com
• bouwenmetstaal.nl
2.15 Disposal
• steel-sci.com
Due to its high value as a resource, steel scrap is not disposed,
but instead fed into a well-established cycle of reuse or
3. LCA: Calculation rules
the steel is shredded and sorted.
3.1 Declared Unit
The declared unit is 1 t of PRS galvanized structural steel. In module C3, shredding and sorting of the disassembled
Declared unit and mass reference product is assumed for the share to be recycled. The recovered
material leaves the product system as 'materials for recycling'.
Name Value Unit
1 % of the shredded/sorted material is considered dust/loss,
Declared unit 1000 kg
which is disposed of in a landfill for inert materials.
Gross density 7850 kg/m3 The net amounts of the metals leaving the product system are
considered as 'use of secondary material' in Module D.
3.2 System boundary
Type of the EPD: cradle to gate with options, with modules C1– As stated above, a reuse/recycling scenario in conformity with
C4, and module D. the European Commission Technical Steel Research (2001) on
steel used in construction has been used. The landfilling of
The production of PRS structural steel (modules A1–A3) shredding/sorting losses is declared in C3. Hence, no impacts
includes raw material extraction, energy generation, waste are declared in module C4.
treatment and all transports up to the factory gate. In
accordance with COUNCIL REGULATION (EU) No 333/2011, Module D contains the benefits beyond the system boundary
secondary steel is modelled as part of the product system from related to the reuse of the steel structure, leading to the
the moment they are available as unmixed scrap. substitution of the production of the corresponding steel
Waste or secondary fuels are not used for production. structure.
It also contains the benefits and loads beyond the system
Module A4 is not declared due to large variances in transport boundary related to the recycling of steel, which results from
distances between the production site and the construction site, the treatment of recycled materials from the point of end-of-
where the product is installed. waste status to the point of substitution (as loads) and the
substitution of primary resources (as benefits).
In module A5, the products are delivered to the construction It also includes the benefits and loads related to the energy
site ready to be installed. Manual installation supported by a recovery from wooden wastes in a municipal waste incineration
diesel-powered mobile crane is assumed, electricity plant as modelled in Module A5.
consumption related to electric drilling machines, screwdrivers, Only net flows leaving the product system are considered in
etc. is considered to be negligible. module D. The recycled content and the assumed processing
The wooden battens used for storage/transport are assumed to losses (e.g., during remelting) are taken from respective
be transported to an incineration plant; the recovered energy is ecoinvent 3 datasets; these parameters are used to estimate
declared as exported energy. the input of secondary material and compare it with the output
flows of the corresponding material.
Modules B1 to B7 are not relevant for the declared products.
3.3 Estimates and assumptions
The indicator values of Modules B1 to B7 are thus 0 and not
No further assumptions and estimates relevant to the result had
declared in the results table.
to be made beyond the points made in chapter 3 and in chapter
4.
In analogy to module A5, manual installation supported by a
diesel-powered mobile crane is assumed (module C1).
3.4 Cut-off criteria
A share of 11 % of dismantled products is re-used in a different
No data available from the company survey was neglected.
location and reaches the end-of-waste stage after dismantling
These include, among other things, material use, energy
(European Commission Technical Steel Research, 2001); the
demand (heat, electricity), wooden battens for
corresponding amount leaves the product system as
storage/transport, consumables in production, waste treatment
'components for reuse'.
and the transport of all inputs and outputs.
With this approach, mass and energy flows below 1 % were
In module C2, the remaining 89 % of the dismantled steel
also accounted for. No processes were neglected that would
construction undergo a recycling (European Commission
have been known to the project managers and would have
Technical Steel Research, 2001) via a recycling platform, where
contributed significantly to the indicators of the impact
4 Environmental Product Declaration - Astron Buildings S.A. - Astron PRS Product (galvanized steel elements made of welded sections)
assessment. No co-products are generated during the production of PRS
structural steel. Sorted production scrap is considered a
3.5 Background data
secondary material with no economic value (so no burdens
Ecoinvent v3.9.1, system model "cut-off by allocated) and considered closed-loop in modules A1–A3 (thus
classification" (2022) is used as the background database. not taken into account in module D.
Economic allocation is applied to the blast furnace process
3.6 Data quality
related to pig iron and raw slag in accordance with the
The foreground data are based on extensive and detailed data
ecoinvent v3.9.1 dataset.
collection at the production site. The foreground data could be
fully linked with corresponding data records from the
No processes were modelled as part of the foreground model
background database ecoinvent v3.9.1.
that would have required an allocation of multi-input processes.
The background data was updated in 2022. Thus, the quality of
Background datasets on municipal waste incineration plants
the foreground and background data can be rated as very
were taken from ecoinvent without any modification.
good.
Allocation of reuse, recycling and recovery was avoided by the
3.7 Period under review
cut-off approach in the foreground model in line with EN 15804.
The LCA data represents the production conditions for the Q4
of year 2021 and Q1–Q3 of year 2022. 3.10 Comparability
Basically, a comparison or an evaluation of EPD data is only
3.8 Geographic Representativeness
possible if all the data sets to be compared were created
Land or region, in which the declared product system is
according to EN 15804 and the building context, respectively
manufactured, used or handled at the end of the product´s
the product-specific characteristics of performance, are taken
lifespan: Germany
into account. Ecoinvent v3.9.1, system model "cut-off by
classification" (2022) is used as the background database.
3.9 Allocation
4. LCA: Scenarios and additional technical information
Characteristic product properties of biogenic carbon Module C2
Note: 1 kg of biogenic carbon is equivalent to 44/12 kg of CO 2 In module C2, the remaining 89 % of the dismantled steel
construction undergo a recycling (European Commission
Information on describing the biogenic carbon content at
Technical Steel Research, 2001) via a recycling platform, where
factory gate
the steel is shredded and sorted.
Name ValueUnit
A default distance of 50 km to the shredding/sorting station is
kg assumed.
Biogenic carbon content in product -
C
Biogenic carbon content in accompanying kg Module C3
2.95
packaging C In module C3, a consumption of 0.015 kWh/kg of electricity for
shredding and sorting and 0.0437 MJ/kg of diesel fuel for
internal logistics are taken into for the shredding and sorting of
disassembled the product (values taken from published IBU
Module A5
EPD on identical product). The recovered material leaves the
In module A5, the products are delivered to the construction
product system as 'materials for recycling'.
site ready to be installed. Manual installation supported by a
1 % of the shredded/sorted material is considered dust/loss,
diesel-powered mobile crane is assumed, electricity
which is disposed of in a landfill for inert materials. A transport
consumption related to electric drilling machines, screwdrivers,
of 30 km.
etc. is considered to be negligible.
The net amounts of the metals leaving the product system are
The wooden battens used for storage/transport are assumed to
considered as 'use of secondary material' in Module D.
be transported 50 km with a lorry with a payload of 16-32 metric
ton, EURO6 to an incineration plant with an efficiency R1>0.6
Module D
(according to CEWEP Energy Report III); the recovered energy
Module D contains the benefits and loads beyond the system
is declared as exported energy; according to the same report,
boundary related to the recycling of metals, which result from
for its quantification, an efficiency of 28.3 % is assumed for the
the treatment of recycled materials from the point of end-of-
production of heat and 14.8 % for the production of electricity
waste status to the point of substitution (as loads) and the
(always referring to the lower heating value of the waste).
substitution of primary resources (as benefits).
It also includes the benefits and loads related to the energy
Module C1
recovery from wooden wastes in a municipal waste incineration
In analogy to module A5, manual installation supported by a
plant as modelled in Module A5.
diesel-powered mobile crane is assumed (module C1).
Only net flows leaving the product system are considered in
Electricity consumption related to electric drilling machines,
module D. The recycled content and the assumed processing
screw drivers, etc. is considered to be negligible.
losses (e.g., during remelting) are taken from respective
A share of 11 % of dismantled products is re-used in a different
ecoinvent 3 datasets; these parameters are used to estimate
location and reaches the end-of-waste stage after dismantling
the input of secondary material and compare it with the output
(European Commission Technical Steel Research, 2001); the
flows of the corresponding material.
corresponding amount leaves the product system as
"components for reuse".
5 Environmental Product Declaration - Astron Buildings S.A. - Astron PRS Product (galvanized steel elements made of welded sections)
5. LCA: Results
DESCRIPTION OF THE SYSTEM BOUNDARY (X = INCLUDED IN LCA; ND = MODULE OR INDICATOR NOT DECLARED; MNR =
MODULE NOT RELEVANT)
Benefits and
Construction loads beyond
Product stage Use stage End of life stage
process stage the system
boundaries
la ire ta m w a Ry lp p u s tro p s n a rT g n iru tc a fu n a M e h t m o rf tro p s n a rTe tis e h t o t e ta g y lb m e s s A e s U e c n a n e tn ia M ria p e R tn e m e c a lp e R tn e m h s ib ru fe R y g re n e la n o ita re p Oe s u re ta w la n o ita re p Oe s u n o itc u rts n o c -e Dn o itilo m e d tro p s n a rT g n is s e c o rp e ts a W la s o p s iD -e s u e R-y re v o c e R-g n ilc y c e Rla itn e to p
A1 A2 A3 A4 A5 B1 B2 B3 B4 B5 B6 B7 C1 C2 C3 C4 D
X X X MND X MND MND MNR MNR MNR MND MND X X X X X
RESULTS OF THE LCA - ENVIRONMENTAL IMPACT according to EN 15804+A2: 1 t of PRS galvanized structural steel
Parameter Unit A1-A3 A5 C1 C2 C3 C4 D
GWP-total kg CO 2 eq 2.55E+03 1.66E+01 5.07E+00 8.23E+00 1.32E+01 0 -1.21E+03
GWP-fossil kg CO 2 eq 2.56E+03 5.89E+00 5.07E+00 8.22E+00 1.32E+01 0 -1.21E+03
GWP-biogenic kg CO 2 eq -1.08E+01 1.08E+01 0 0 0 0 0
GWP-luluc kg CO 2 eq 1.49E+00 9.48E-04 5.71E-04 4.06E-03 1.54E-03 0 -2.72E-01
ODP kg CFC11 eq 5.39E-05 9.86E-08 8.06E-08 1.79E-07 1.67E-07 0 -2.54E-05
AP mol H+ eq 1.08E+01 4.87E-02 4.7E-02 1.8E-02 5.81E-02 0 -5.08E+00
EP-freshwater kg P eq 1.15E-01 2.48E-05 1.83E-05 6.68E-05 4.63E-04 0 -5.45E-02
EP-marine kg N eq 2.25E+00 2.22E-02 2.18E-02 4.42E-03 2.14E-02 0 -1.04E+00
EP-terrestrial mol N eq 2.6E+01 2.41E-01 2.37E-01 4.61E-02 2.36E-01 0 -1.21E+01
kg NMVOC
POCP 1.19E+01 7.28E-02 7.01E-02 2.79E-02 7.06E-02 0 -6.28E+00
eq
ADPE kg Sb eq 4.53E-02 4.4E-06 1.77E-06 2.69E-05 9.57E-06 0 -1.12E-02
ADPF MJ 3.03E+04 7.8E+01 6.64E+01 1.17E+02 1.94E+02 0 -1.16E+04
m3 world eq
WDP 8.23E+02 1.87E-01 1.43E-01 4.81E-01 3.71E-01 0 -1.49E+02
deprived
GWP = Global warming potential; ODP = Depletion potential of the stratospheric ozone layer; AP = Acidification potential of land and water; EP =
Eutrophication potential; POCP = Formation potential of tropospheric ozone photochemical oxidants; ADPE = Abiotic depletion potential for non-fossil
resources; ADPF = Abiotic depletion potential for fossil resources; WDP = Water (user) deprivation potential)
RESULTS OF THE LCA - INDICATORS TO DESCRIBE RESOURCE USE according to EN 15804+A2: 1 t of PRS galvanized
structural steel
Parameter Unit A1-A3 A5 C1 C2 C3 C4 D
PERE MJ 2.93E+03 1.13E+02 3.73E-01 1.81E+00 1.22E+00 0 -9.91E+02
PERM MJ 1.12E+02 -1.12E+02 0 0 0 0 0
PERT MJ 3.04E+03 5.72E-01 3.73E-01 1.81E+00 1.22E+00 0 -9.91E+02
PENRE MJ 3.03E+04 7.8E+01 6.64E+01 1.17E+02 1.94E+02 0 -1.15E+04
PENRM MJ 0 0 0 0 0 0 0
PENRT MJ 3.03E+04 7.8E+01 6.64E+01 1.17E+02 1.94E+02 0 -1.15E+04
SM kg 1.68E+02 0 0 0 0 0 -1.85E+01
RSF MJ 0 0 0 0 0 0 0
NRSF MJ 0 0 0 0 0 0 0
FW m3 3.33E+01 1.31E-02 1.05E-02 3.02E-02 3.91E-02 0 -1.25E+01
PERE = Use of renewable primary energy excluding renewable primary energy resources used as raw materials; PERM = Use of renewable primary
energy resources used as raw materials; PERT = Total use of renewable primary energy resources; PENRE = Use of non-renewable primary energy
excluding non-renewable primary energy resources used as raw materials; PENRM = Use of non-renewable primary energy resources used as raw
materials; PENRT = Total use of non-renewable primary energy resources; SM = Use of secondary material; RSF = Use of renewable secondary fuels;
NRSF = Use of non-renewable secondary fuels; FW = Use of net fresh water
RESULTS OF THE LCA – WASTE CATEGORIES AND OUTPUT FLOWS according to EN 15804+A2:
1 t of PRS galvanized structural steel
Parameter Unit A1-A3 A5 C1 C2 C3 C4 D
HWD kg 3.69E-01 5.21E-04 4.47E-04 7.43E-04 5.26E-04 0 -1.25E-01
NHWD kg 1.43E+03 6E-01 1.18E-01 5.85E+00 9.33E+00 0 -5.17E+02
RWD kg 8.96E-02 2.03E-05 1.22E-05 6.7E-05 9.95E-04 0 1.19E-02
CRU kg 0 0 1.2E+02 0 0 0 0
MFR kg 0 0 0 0 8.81E+02 0 0
MER kg 0 0 0 0 0 0 0
EEE MJ 0 1.64E+01 0 0 0 0 0
EET MJ 0 3.13E+01 0 0 0 0 0
6 Environmental Product Declaration - Astron Buildings S.A. - Astron PRS Product (galvanized steel elements made of welded sections)
HWD = Hazardous waste disposed; NHWD = Non-hazardous waste disposed; RWD = Radioactive waste disposed; CRU = Components for re-use;
MFR = Materials for recycling; MER = Materials for energy recovery; EEE = Exported electrical energy; EET = Exported thermal energy
RESULTS OF THE LCA – additional impact categories according to EN 15804+A2-optional:
1 t of PRS galvanized structural steel
Parameter Unit A1-A3 A5 C1 C2 C3 C4 D
Disease
PM 1.85E-04 1.36E-06 1.31E-06 6.1E-07 1.08E-06 0 -8.15E-05
incidence
IR kBq U235 eq 7E+01 2.04E-02 1.36E-02 5.92E-02 4.17E-01 0 5.6E+00
ETP-fw CTUe 1.76E+04 3.76E+01 3.17E+01 5.77E+01 4.44E+01 0 -2.04E+03
HTP-c CTUh 1.74E-05 1.89E-09 1.55E-09 3.75E-09 2.85E-09 0 6.84E-06
HTP-nc CTUh 3.61E-05 1.85E-08 1.08E-08 8.29E-08 8.21E-08 0 -8.75E-06
SQP SQP 1.1E+04 1.04E+01 4.47E+00 7.06E+01 1.74E+01 0 -3.36E+03
PM = Potential incidence of disease due to PM emissions; IR = Potential Human exposure efficiency relative to U235; ETP-fw = Potential comparative
Toxic Unit for ecosystems; HTP-c = Potential comparative Toxic Unit for humans (cancerogenic); HTP-nc = Potential comparative Toxic Unit for humans
(not cancerogenic); SQP = Potential soil quality index
Disclaimer 1 – for the indicator “Potential Human exposure efficiency relative to U235”. This impact category deals mainly with the
eventual impact of low-dose ionizing radiation on human health of the nuclear fuel cycle. It does not consider effects due to possible
nuclear accidents, occupational exposure or radioactive waste disposal in underground facilities. Potential ionizing radiation from the
soil, radon and from some construction materials is also not measured by this indicator.
Disclaimer 2 – for the indicators “abiotic depletion potential for non-fossil resources”, “abiotic depletion potential for fossil resources”,
“water (user) deprivation potential, deprivation-weighted water consumption”, “potential comparative toxic unit for ecosystems”,
“potential comparative toxic unit for humans – cancerogenic”, “Potential comparative toxic unit for humans - not cancerogenic”,
“potential soil quality index”. The results of this environmental impact indicator shall be used with care as the uncertainties on these
results are high as there is limited experience with the indicator.
6. LCA: Interpretation
Figure 1 illustrates the relative contributions of the different
modules along the life cycle of the declared products The LCA is dominated by the manufacture of the product
(contribution of modules A1–C4 = 100 %). (modules A1–A3).
The benefits and burdens outside the product system vary in
significance depending on the indicator and fluctuate between -
20 % and -50 %.
The use of renewable primary energy is mainly caused by the
share of renewable energy in the electricity mix, thus the
production stage is the main driver of this impact category; the
same holds also for the use of non-renewable primary energy.
Material use of primary energy is comparably small and related
to the use of wooden battens used for transport and storage.
The material use of primary energy is transferred to its energy
use when the materials containing primary energy are
incinerated with energy recovery; the material use of primary
energy is subtracted from the material use indicator when the
materials containing primary energy are recycled. Non-
hazardous waste as the quantitatively most relevant waste
flows is mainly caused during mining and processing of metal
ores and related to the disposal of road infrastructure;
Figure 1: Relative contributions of the different life cycle hazardous and radioactive waste are mainly caused by the
stages for taylor-made welded galvanized beams (PRS) nuclear power in the electricity mix.
(modules A1–C4 = 100 %)
7. Requisite evidence
7.1 Weathering For complete chemical weathering, recent publications (see
When exposed to the elements, the surfaces of hot-dip Hullmann 2003) quote corrosion rates for zinc of 3.0 g/m2*a
galvanized steel components become naturally covered in a (corresponding to approx. 0.5 µm/a).
protective layer known as patina. Patina is extremely durable Recent studies (BAST 2008 and Schröder 2013) examined hot-
and thus provides for exceptionally effective protection against dip galvanized steel crash barriers along the German Federal
corrosion, lasting several decades. Motorway BAB 4 and detected no measurable loss of thickness
At the same time, it protects the zinc coating, so that it remains of the zinc coating due to chemical weathering after 10 years of
intact for a long period of time. exposure to the elements.
The ever more stringent air quality improvement measures (in Chemical weathering can thus be assumed to be minimal and
particular the desulphurisation of power plant and engine fuels) therefore negligible, even over several years and under
have a major positive impact on the reduction of chemical increased corrosion stress such as along motorways (where
weathering of zinc coatings. Schröder 2013 reports of zinc deicing salt is used during the winter months).
coating depletion rates of up to 4.7 µm/a observed in the 1970s
in hot-dip galvanized steel crash barriers.
7 Environmental Product Declaration - Astron Buildings S.A. - Astron PRS Product (galvanized steel elements made of welded sections)
8. References
Product category rules of IBU ISO 14044
EN ISO 14044:2006-07, Environmental management - Life
IBU (2021) cycle assessment - Requirements and guidance (ISO
IBU (2021): PCR Part A: Calculation rules for the life cycle 14044:2006); German and English versions EN ISO
assessment and requirements on the project report according 14044:2006.
to EN 15804+A2. Version 1.3, Institut Bauen und Umwelt e.V.,
Berlin. ISO 14713-1
DIN EN ISO 14713-1:2017-08, Zinc coatings - Guidelines and
IBU (2021) recommendations for the protection against corrosion of iron
IBU (2021): General Instructions for the EPD Programme of the and steel in structures - Part 1: General principles of design and
Institut Bauen und Umwelt e.V. (General Instructions for the corrosion resistance (ISO 14713-1:2017); German version EN
IBU EPD Programme). Version 2.0, Institut Bauen unf Umwelt, ISO 14713-1:2017.
Berlin.
EN 15804
IBU (2023) DIN EN 15804+A2:2022-03, Sustainability of construction
IBU (2023): PCR Part B: Requirements on the EPD for works - Environmental product declarations - Core rules for the
structural steel. Version 2023/04, Institut Bauen und Umwelt product category construction products; German version EN
e.V., Berlin. 15804:2012+A2:2019 + AC:2021.
Standards and legal documents EN 16485
DIN EN 16485:2014-07, Round and sawn timber -
EN 1090-1 Environmental Product Declarations - Product category rules
DIN EN 1090-1:2012-02, Execution of steel structures and for wood and wood-based products for use in construction;
aluminium structures - Part 1: Requirements for conformity German version EN 16485:2014.
assessment of structural components; German version EN
1090-1:2009+A1:2011. ECHA candidate list
The Candidate List of substances of very high concern,
EN 1090-2 available via https://echa.europa.eu/nl/-/four-newsubstances-
DIN EN 1090-2:2012-02, Execution of steel structures and added-to-the-candidate-list.
aluminium structures - Part 2: Technical requirements for steel
structures; German version EN 1090-2:2018. ETA-18/1027
ETA-18/1027 of 19 November 2018 for Metal Frame Building
EN ISO 1461 Kits by Astron Buildings S.A.
DIN EN ISO 1461:2009-10, Hot dip galvanized coatings on
fabricated iron and steel articles - Specifications and test Regulation on biocidal products
methods (ISO 1461:2009); German version EN ISO 1461:2009. REGULATION (EU) No 528/2012 OF THE EUROPEAN
PARLIAMENT AND OF THE COUNCIL of 22 May 2012
EN 1993 concerning the making available on the market and use of
DIN EN 1993-1-1:2010-12, Eurocode 3: Design of steel biocidal products.
structures - Part 1-1: General rules and rules for buildings;
German version EN 1993-1-1:2005 + AC:2009. Regulation (EU) Nr. 305/2011(CPR)
REGULATION (EU) No 305/2011 OF THE EUROPEAN
EN 1994 PARLIAMENT AND OF THE COUNCIL of 9 March 2011 laying
DIN EN 1994-1-1:2010-12, Eurocode 4: Design of composite down harmonised conditions for the marketing of construction
steel and concrete structures - Part 1-1: General rules and rules products and repealing Council Directive 89/106/EEC.
for buildings; German version EN 1994-1-1:2004 + AC:2009.
Regulation on the European Waste List
ISO 9001 http://www.gesetze-im-internet.de/avv/anlage.html.
DIN EN ISO 9001:2015, Quality management systems -
Requirements. Additional references
EN 10025 BAST (2008)
DIN EN 10025-1:2005-02, Hot rolled products of structural BAST (2008): Coil-coated safety rails; German Federal
steels - Part 1: General technical delivery conditions; German Highway Research Institute (BASt) Bergisch-Gladbach 2008.
version EN 10025-1:2004.
Bundesministerium für Umwelt, Naturschutz, Bau und
ISO 12944-2 Reaktorsicherheit
DIN EN ISO 12944-2:2018-04, Paints and varnishes - Instrumente zur Wiederverwendung von Bauteilen und
Corrosion protection of steel structures by protective paint hochwertigen Verwertung von Baustoffen',
systems - Part 2: Classification of environments (ISO 12944- (Umweltforschungsplan des Bundesministeriums für Umwelt,
2:2017); German version EN ISO 12944-2:2017. Naturschutz, Bau und Reaktorsicherheit ; Forschungskennzahl
3712 32 319; UBA-FB 002208).
ISO 14025
ISO 14025:2006-07, Environmental labels and declarations - CEWEP Energy Report III (2013)
Type III Environmental declarations - Principles and Reimann D.O. (2013): CEWEP Energy Report III (Status 2007
procedures. – 2010); Results of Specific Data for Energy, R1 Plant
Efficiency Factor and NCV of 314 European Waste-to-Energy
8 Environmental Product Declaration - Astron Buildings S.A. - Astron PRS Product (galvanized steel elements made of welded sections)
(WtE) Plants. CEWEP, Würzburg/Brussels, 2013. research.
DASt-Guideline 022 Hullmann 2003
Institut Feuerverzinken (2016): Feuerverzinken von tragenden Hullmann H. (2003): Natürlich oxidierende Metalloberflächen;
Stahlbauteilen. DASt-Richtlinie 022 und Erläuterung zur DASt- Umweltauswirkungen beim Einsatz von Kupfer und Zink in
Richtlinie 022. Institut Feuerverzinken, Ausgabe Juni 2016. Gebäudehüllen; 2003, Stuttgart, Fraunhofer ISB-Verlag, ISBN:
3-8167-6218-2.
ecoinvent v3.9.1
ecoinvent v3.9.1, LCA database, 12/2022. Ecoinvent centre, Schröder 2013
Zürich. Schröder M. (2012): Korrosionsbeständigkeit von
diskontinuierlich und kontinuierlich verzinkten Schutzplanken,
European Commission Technical Steel Research (2001) Vortrag anlässlich EGGA-Assembly, 10.-13. Juni 2013,
Sansom M., Meijer J. (2001): Life-cycle assessment; (LCA) for Dresden.
steel construction, European Commission technical steel
9 Environmental Product Declaration - Astron Buildings S.A. - Astron PRS Product (galvanized steel elements made of welded sections)
Publisher
Institut Bauen und Umwelt e.V. +49 (0)30 3087748- 0
Hegelplatz 1 info@ibu-epd.com
10117 Berlin www.ibu-epd.com
Germany
Programme holder
Institut Bauen und Umwelt e.V. +49 (0)30 3087748- 0
Hegelplatz 1 info@ibu-epd.com
10117 Berlin www.ibu-epd.com
Germany
Author of the Life Cycle Assessment
Dr. Frank Werner - Umwelt & Entwicklung + 41 (0)44 241 39 06
Kammelenbergstrasse 30 frank@frankwerner.ch
9011 St. Gallen http://www.frankwerner.ch/
Switzerland
Owner of the Declaration
Astron Buildings S.A +352 802 91-1
Route d’Ettelbruck 34 info@astron.biz
9230 Diekirch www.astron.biz
Luxembourg
10 Environmental Product Declaration - Astron Buildings S.A. - Astron PRS Product (galvanized steel elements made of welded sections)
