ENVIRONMENTAL PRODUCT DECLARATION
as per ISO 14025 and EN 15804+A2
Owner of the Declaration Uzin Utz SE
Publisher Institut Bauen und Umwelt e.V. (IBU)
Programme holder Institut Bauen und Umwelt e.V. (IBU)
Declaration number EPD-UZI-20230498-IBC1-EN
Issue date 29.01.2024
Valid to 28.01.2029
Fabric Tape
Sifloor AG
www.ibu-epd.com | https://epd-online.com
1. General Information
Sifloor AG Fabric Tape
Programme holder Owner of the declaration
IBU – Institut Bauen und Umwelt e.V. Uzin Utz SE
Hegelplatz 1 Dieselstraße 3
10117 Berlin 89079 Ulm
Germany Germany
Declaration number Declared product / declared unit
EPD-UZI-20230498-IBC1-EN 1 m2 of: Fabric Tape
This declaration is based on the product category rules: Scope:
Dispersion adhesives and primers for floor coverings, 01.08.2021 This Environmental Product Declaration is an average EPD for dry
(PCR checked and approved by the SVR) adhesives covering the products: UZIN Sigaway Orginal, UZIN Sigaway
Tape.
The data provided in this EPD refers to the arithmetic mean of the products
Issue date mentioned. All products covered by this EPD are manufactured at the
Sifloor AG plant in Sursee, Switzerland.
29.01.2024
The owner of the declaration shall be liable for the underlying information
and evidence; the IBU shall not be liable with respect to manufacturer
information, life cycle assessment data and evidences.
Valid to
28.01.2029 The EPD was created according to the specifications of EN 15804+A2. In
the following, the standard will be simplified as EN 15804.
Verification
The standard EN 15804 serves as the core PCR
Independent verification of the declaration and data according to ISO
14025:2011
internally X externally
Dipl.-Ing. Hans Peters
(Chairman of Institut Bauen und Umwelt e.V.)
Florian Pronold Matthias Schulz,
(Managing Director Institut Bauen und Umwelt e.V.) (Independent verifier)
1 Environmental Product Declaration - Sifloor AG - Fabric Tape
2. Product
requirements. Furthermore, these products are awarded with
2.1 Product description/Product definition the Blue Angel (DE-UZ 113) due to their low emissions.
This EPD comprises dry adhesives of the product category:
Fabric-Tapes. All products considered here are based on the REACH regulation:
switchTec dry adhesive technology. This is a technology for
floor bonding and fulfils the function of liquid adhesives as an Does this product/article/at least one partial article contains
alternative in flooring technology. substances listed in the candidate list (date: 01.01.2024)
The following products can be assigned to this EPD: exceeding 0.1 percentage by mass?
• UZIN Sigaway Orginal NO
• UZIN Sigaway Tape
• UZIN Pluratex Does this product/article/at least one partial article contains
other CMR substances in categories 1A or 1B which are not on
For the use and application of the product the respective the candidate list, exceeding 0.1 percentage by mass?
national provisions at the place of use apply, in Germany for NO
example the building codes of the federal states and the
corresponding national specifications. Were biocide products added to this construction product or
has it been treated with biocide products (this then concerns a
2.2 Application treated product as defined by the (EU) Ordinance on Biocide
The different fabric tapes are specially adapted to different Products No. 528/2012)?
substrates and floor coverings and are suitable for full-surface NO
bonding of floor coverings. Substrates that meet the
requirements of DIN 18365 are suitable for the use of dry Information on hazardous substances (if any) contained in this
adhesives after levelling. product can be found in the product specific Safety Data sheet.
The latest version is available at our Website:
2.3 Technical Data https://int.uzin.com/
The various tapes are specially adapted to different substrates
and floor coverings to comply with their requirements.
Constructional data
2.6 Manufacture
Name Value Unit
The ingredients of the adhesive component are first added
Dimensional changes (in transverse direction) together according to the corresponding formula and mixed
acc. to ISO 22633 (Dispersion adhesives for under continuous stirring. In two steps, the adhesive
textile and elastic floor coverings, not applicable max. component is then first applied to the carrier material on one
<0.2%
for polyvinyl chloride floor coverings, rubber floor % side and dried in the drying line. The process is then repeated
coverings, smooth polyolefin floor coverings, for the other side. Some substrates are such that the adhesive
textile floor coverings) component penetrates the substrate. In this case, one coating
Dimensional changes acc. to ISO 22635 cycle is sufficient and the second adhesive coating step is
(Dispersion adhesives for textile and elastic floor max. omitted. In order to prevent the fabric tape from sticking when it
<0.2%
coverings, (not applicable for linoleum or textile % is rolled up, a protective paper (liner) is applied to one of the
floor coverings) adhesive sides.
Other constructional data are not relevant for this product. 2.7 Environment and health during manufacturing
Apart from the standard precautions for occupational hygiene
Performance data of the product with respect to its
and safety, there are no special protective precautions to be
characteristics in accordance with the relevant technical
observed during production.
provision (no CE-marking).
2.8 Product processing/Installation
2.4 Delivery status
Dry adhesives are applied by hand on appropriately prepared
All products covered by this EPD are delivered ready to use.
substrates. To do so, first the edge tape is installed along walls
The content of one packaging unit for UZIN Sigaway Original is
and doors. Then the tapes are rolled out to an area to be
sufficient for 25 m2, for UZIN Sigaway Tape it is sufficient for installed and rubbed in thoroughly with a textile cork rubbing
1,25 m2 and for UZIN Pluratex it is sufficient for 22,5 m2. board. Following the tape is cut to size with a hook knife.
Afterwards, the protective paper on the opposite side is peeled
2.5 Base materials/Ancillary materials
off, revealing a second adhesive side. In the last step, the floor
Dry adhesives in general consist of a carrier material with a
covering can be applied to the second adhesive side by
self-adhesive layer on both sides. On average, the film tapes
applying pressure on it.
covered by this EPD are composed of:
Name Value Unit 2.9 Packaging
Synthetic polymer dispersion (solid content) 40 - 60 % All products considered in this EPD are packed in a cardboard
packaging. Emptied cores and cardboard packaging are
Water 20 - 35 %
recyclable. The weight and shape of the packaging are different
Additives <0.3 %
for the products considered here. More details can be found
Liner (protective paper) 10 - 35 % under Section 2.4.
Carrier material 5 - 15 %
2.10 Condition of use
UZIN Sigaway Orginal and UZIN Sigaway Tape are very low in
The substantial composition during the use phase refers to the
volatile organic compound (VOC) emission. They are certified
composition during the manufacturing. Compared to liquid
as EMICODE EC1 Plus according to the EMICODE
2 Environmental Product Declaration - Sifloor AG - Fabric Tape
adhesives, dry adhesives do not harden through chemical primarily determined by the type and nature of the installed
reactions, but are permanently adhesive and do not dry out. floor covering or insulation layers. Therefore, the fire resistance
class of the floor covering according to EN 13501 must be
2.11 Environment and health during use taken into account when assessing the fire behaviour. The fire
UZIN Sigaway Orginal and UZIN Sigaway Tape have been classification of the floor covering to be installed will be
awarded the emission label EMICODE EC 1 PLUS "very low maintained when installed on switchTec dry adhesives.
emission" and the Blue Angel (DE-UZ 113). With the emission Water
label, these dry adhesives contribute to preserving a healthy Excessive amounts of water can damage the substrate or the
indoor climate. Details on the individual criteria of the floor covering. When the dry adhesive comes into contact with
EMICODE can be found under point 7 Requisite Evidence. water, the adhesive strength is weakened and returns to full
Therefore UZIN Sigaway Orginal and UZIN Sigaway Tape also strength after the water has fully evaporated. No substances
meet the highest DGNB Quality Level 4. Furthermore, the are washed out that could be hazardous to water.
products contribute to further green building rating systems
such as LEED and BREEAM. UZIN Sigaway Orginal and UZIN Mechanical destruction
Sigaway Tape are also provided with the Ü-mark. Not of relevance.
2.14 Re-use phase
2.12 Reference service life Since adhesive residues may remain on the covering and the
The service life of dry adhesives depends on the service life of substrate, it is usually disposed of together, respectively. The
the floor covering. In turn, the service life of different floor re-use of the tapes covered by this EPD is not possible.
coverings show a high variability (10-50 years according to the
table "Service lives of components for life cycle assessment 2.15 Disposal
according to Assessment System for Sustainable Building The EWC waste code in accordance with the European Waste
(BNB)"; BBSR: Bundesinstitut für Bau-, Stadt- und Catalogue / List of Waste Ordinance for cured dispersion waste
Raumforschung; www.nachhaltigesbauen.de/baustoff- bears the EWC waste code 080410 (adhesive and sealing
undgebaeudedaten/nutzungsdauern-von-bauteilen.html)) compound waste). Material residues can be disposed of as
Therefore, the specification of a reference service life according household waste.
to ISO 15686 is not possible.
2.16 Further information
2.13 Extraordinary effects Product and safety data sheet, EMICODE EC 1 PLUS and Blue
Fire Angel certificate, general building authority approval and further
There are no normative requirements for fire protection for this information at https://int.uzin.com/.
product group. The fire behaviour of the floor construction is
3. LCA: Calculation rules
indicators is given in Chapter 6.
3.1 Declared Unit
This declaration is an average EPD and refers to 1 m2 of the 3.2 System boundary
fabric tapes UZIN Sigaway Orginal, UZIN Sigaway Tape and Type of EPD: Cradle to gate with options, modules C1–C4, and
UZIN Pluratex, manufactured by SIFLOOR AG at the Sursee module D (A1–A3 + C + D and additional modules). The
plant. All values stated in this EPD represent the arithmetic additional modules are A4 and A5. The underlying LCA
mean of the individual values of the products. The products addresses all life cycle stages of the average product. The
mentioned are manufactured at the same plant, fulfil the same other life cycle stages are not relevant for the product class and
or a comparable function and differ only slightly in their no environmental impacts occur in these. The following
formulation; other life cycle phases are the same, such as activities are covered by the relevant modules:
production. The declared unit of 1 m2 was chosen as the • A1: Production of raw and auxiliary materials
operating data is recorded either per linear metre [m] or per • A2: Transport of raw and auxiliary materials to the plant
square metre [m2] and the sales unit is also given in m2. Using • A3: Production in the plant (incl. provision of energy and
the conversion factor of the average mass per square metre, waste treatment) and the manufacture of the packaging
the data given can be related to 1 kg. • A4: Transport of the packed product to the construction
site
Declared unit and mass reference
• A5: Installation of the product and disposal of the
Name Value Unit
packaging and waste produced during installation
Declared Unit 1 m2 (including the protective paper)
Gross density 1 - 1.5 kg/m3 • C1: Manual removal of the product
• C2: Transport for disposal
Grammage (average over all products
0.310 kg/m2 • C3: As a worst-case scenario thermal treatment of the
considered)
product in an incineration plant is modelled as end-of-
Layer thickness (average over all products
0.0003 m life scenario
considered)
• C4: Not relevant because the product is incinerated
The representativeness of the average LCA values is rated as (respective impacts declared in C3)
good. Comparability with regard to temporal, geographical and • D: Credits resulting from thermal utilisation of the
technological factors is ensured by the fact that all the products product and packaging waste
considered here were manufactured in the same plant using For the environmental impact, the use of green electricity was
the same machinery, while the same reference year was calculated taking into account the residual electricity mix for the
utilised. Differences may arise in the exact composition of the remaining electricity. The proportion of the on-site electricity
applied adhesive and its coating thickness, as well as the demand covered by green electricity in the total on-site
substrate material used. electricity demand is 100 %.
Further information regarding the variability of specific impact
3 Environmental Product Declaration - Sifloor AG - Fabric Tape
3.3 Estimates and assumptions
No material loss was assumed in module A5 (installation), as
this is strongly dependent on the application procedure. In
order to determine the environmental burdens caused by the
compensation of the additional material effort due to the
material loss, the following scheme can be used: The material
loss expressed as a percentage [%] is multiplied by the
indicator values from modules A1-A4 and C3 and added to
module A5. A subtraction of the indicator values from modules
A1-A4 and C3 is not necessary, as only the additional material
effort to compensate for the material loss is considered.
As end-of-life assumption for the packaging and the product, a
100 % thermal treatment scenario was chosen, respectively.
Since the products considered in this EPD are delivered in
different packaging, the packaging with the least favourable
ratio of packaging weight to product weight was used for the
calculation.
3.4 Cut-off criteria
The common rules according to ISO 14044 were applied as
cut-off criteria. These apply to the entire product system as well
as to individual process modules and take into account mass,
energy and environmental relevance. All inputs were included
in the LCA that are more than 1 % with regard to the total
impact of an impact category. Overall, no more than 5 % of the
flows were neglected with regard to the cut-off criteria.
3.5 Background data
Factory-specific data was used for the production processes.
For all other life cycle phases, data sets from Sphera Managed
LCA Content (Content Version 2023.2) were used. The LCA
model was created in the software LCA for Experts (Version 10)
(former GaBi).
3.6 Data quality
The data quality can be classified as good. The plant-specific
data refer to the year 2022. All remaining data originate from
the above-mentioned database, the contents of which are
regularly reviewed to ensure their currency. Thus, the data used
for the life cycle assessment are representative. For some input
materials, proxy datasets had to be used. All background
datasets used are less than 10 years old. Data sets are
complete and comply with the system boundaries and the cut-
off rules for inputs and outputs. The data quality thus meets the
requirements of PCR Part A.
3.7 Period under review
The year 2022 is used as the reference year.
3.8 Geographic Representativeness
Land or region, in which the declared product system is
manufactured, used or handled at the end of the product´s
lifespan: Europe
3.9 Allocation
Site-specific operating data was distributed to the different
products according to the machine utilisation.
3.10 Comparability
Basically, a comparison or an evaluation of EPD data is only
possible if all the data sets to be compared were created
according to EN 15804 and the building context, respectively
the product-specific characteristics of performance, are taken
into account. The background database is used from Sphera
Managed LCA Content. In this EPD, dry adhesives are
considered. These differ from liquid dispersion adhesives in
their specific characteristics of performance and response to
(punctual) stresses, so a direct comparison is not possible.
4 Environmental Product Declaration - Sifloor AG - Fabric Tape
4. LCA: Scenarios and additional technical information
No material loss was assumed in module A5 (installation), as
Characteristic product properties of biogenic carbon this is strongly dependent on the application procedure. In
(A1-A3) order to determine the environmental burdens caused by the
compensation of the additional material effort due to the
Note: 1 kg of biogenic carbon is equivalent to 44/12 kg of CO 2. material loss, the following scheme can be used: The material
loss expressed as a percentage [%] is multiplied by the
Information on describing the biogenic carbon content at
indicator values from modules A1-A4 and C3 and added to
factory gate
module A5. A subtraction of the indicator values from modules
Name Value Unit
A1-A4 and C3 is not necessary, as only the additional material
Biogenic carbon content in product (arithmetic 4.70E- kg effort to compensate for the material loss is considered.
mean) 02 C The protective paper, attached to the product is disposed of
Biogenic carbon content in accompanying 2.01E- kg during the installation phase. Thermal treatment was assumed
packaging 02 C as a worst-case scenario.
In the following, the technical scenario information is presented, End of life (C1-C4)
which enables a better understanding of the declared modules. Name ValueUnit
Transport to the building site (A4) Collected as mixed construction waste (arithmetic
0.22 kg
The transport was divided into two phases, which best mean)
correspond to the actual situation. In the first stage, the product Reuse - kg
is transported to a wholesaler by a large truck. The second Recycling - kg
stage represents the transport from the wholesaler to the
Energy recovery 100 %
construction site, which is mostly done by the craftsman with a
Landfilling 0 %
small truck.
Name Value Unit The difference in mass between the product shipped and the
product installed and thus to be disposed of in C3 differs due to
Transport distance (Stage 1) 450 km
the protective paper which is removed during installation. The
Gross weight (Stage 1) 34 - 40 t
waste treatment of the protective paper is declared in module
Payload capacity (Stage 1) 27 t A5.
Utilisation by mass (Stage 1) 0.61
------------------------------- ----------- ----------- -----
Transport distance (Stage 2) 50 km
Gross weight (Stage 2) 7.5 - 12 t
Payload capacity (Stage 2) 5 t
Utilisation by mass (Stage 2) 0.61
Installation into the building (A5)
Name ValueUnit
Auxiliary - kg
Water consumption - m3
Other resources - kg
Electricity consumption - kWh
Other energy carriers - MJ
Material loss - kg
Output substances following waste treatment on
0.09 kg
site
Dust in the air - kg
VOC in the air - kg
5 Environmental Product Declaration - Sifloor AG - Fabric Tape
5. LCA: Results
DESCRIPTION OF THE SYSTEM BOUNDARY (X = INCLUDED IN LCA; MND = MODULE OR INDICATOR NOT DECLARED; MNR
= MODULE NOT RELEVANT)
Benefits and
Construction loads beyond
Product stage Use stage End of life stage
process stage the system
boundaries
la ire ta m w a Ry lp p u s tro p s n a rT g n iru tc a fu n a M e h t m o rf tro p s n a rTe tis e h t o t e ta g y lb m e s s A e s U e c n a n e tn ia M ria p e R tn e m e c a lp e R tn e m h s ib ru fe R y g re n e la n o ita re p Oe s u re ta w la n o ita re p Oe s u n o itc u rts n o c -e Dn o itilo m e d tro p s n a rT g n is s e c o rp e ts a W la s o p s iD -e s u e R-y re v o c e R-g n ilc y c e Rla itn e to p
A1 A2 A3 A4 A5 B1 B2 B3 B4 B5 B6 B7 C1 C2 C3 C4 D
X X X X X MND MND MNR MNR MNR MND MND X X X MND X
RESULTS OF THE LCA - ENVIRONMENTAL IMPACT according to EN 15804+A2: 1 m^2 Fabric Tapes
Parameter Unit A1-A3 A4 A5 C1 C2 C3 D
GWP-total kg CO 2 eq 7.11E-01 1.45E-02 1.99E-01 0 4.77E-04 2.78E-01 -1.15E-01
GWP-fossil kg CO 2 eq 9.47E-01 1.43E-02 1.17E-02 0 4.71E-04 9.61E-02 -1.15E-01
GWP-biogenic kg CO 2 eq -2.44E-01 3.32E-05 1.87E-01 0 1.09E-06 1.81E-01 -5.19E-04
GWP-luluc kg CO 2 eq 8.59E-03 1.34E-04 3.69E-06 0 4.43E-06 5.74E-06 -7.43E-06
ODP kg CFC11 eq 6.8E-09 1.27E-15 2.89E-14 0 4.18E-17 5.05E-14 -8.88E-13
AP mol H+ eq 2.49E-03 5.03E-05 7.84E-05 0 1.64E-06 1.45E-04 -1.42E-04
EP-freshwater kg P eq 9.26E-06 5.29E-08 1.45E-08 0 1.74E-09 2.8E-08 -1.83E-07
EP-marine kg N eq 8.25E-04 2.32E-05 3.01E-05 0 7.57E-07 5.64E-05 -4.18E-05
EP-terrestrial mol N eq 7.81E-03 2.61E-04 3.5E-04 0 8.51E-06 6.43E-04 -4.48E-04
kg NMVOC
POCP 2.26E-03 4.54E-05 7.86E-05 0 1.48E-06 1.47E-04 -1.17E-04
eq
ADPE kg Sb eq 3.01E-06 9.42E-10 2.6E-10 0 3.1E-11 4.36E-10 -8.13E-09
ADPF MJ 2.18E+01 1.97E-01 7.75E-02 0 6.5E-03 1.34E-01 -2.12E+00
m3 world eq
WDP 1.34E-01 1.67E-04 2.24E-02 0 5.51E-06 3.47E-02 -1.08E-02
deprived
GWP = Global warming potential; ODP = Depletion potential of the stratospheric ozone layer; AP = Acidification potential of land and water; EP =
Eutrophication potential; POCP = Formation potential of tropospheric ozone photochemical oxidants; ADPE = Abiotic depletion potential for non-fossil
resources; ADPF = Abiotic depletion potential for fossil resources; WDP = Water (user) deprivation potential)
RESULTS OF THE LCA - INDICATORS TO DESCRIBE RESOURCE USE according to EN 15804+A2: 1 m^2 Fabric Tapes
Parameter Unit A1-A3 A4 A5 C1 C2 C3 D
PERE MJ 4.63E+00 1.4E-02 1.8E+00 0 4.6E-04 6.24E-01 -6.06E-01
PERM MJ 2.38E+00 0 -1.78E+00 0 0 -5.94E-01 0
PERT MJ 7E+00 1.4E-02 2E-02 0 4.6E-04 3E-02 -6.06E-01
PENRE MJ 1.63E+01 1.98E-01 3.84E-01 0 6.52E-03 5.4E+00 -2.12E+00
PENRM MJ 5.57E+00 0 -3.06E-01 0 0 -5.26E+00 0
PENRT MJ 2.19E+01 1.98E-01 7.8E-02 0 6.52E-03 1.4E-01 -2.12E+00
SM kg 0 0 0 0 0 0 0
RSF MJ 0 0 0 0 0 0 0
NRSF MJ 0 0 0 0 0 0 0
FW m3 5.86E-03 1.54E-05 5.29E-04 0 5.07E-07 8.19E-04 -4.91E-04
PERE = Use of renewable primary energy excluding renewable primary energy resources used as raw materials; PERM = Use of renewable primary
energy resources used as raw materials; PERT = Total use of renewable primary energy resources; PENRE = Use of non-renewable primary energy
excluding non-renewable primary energy resources used as raw materials; PENRM = Use of non-renewable primary energy resources used as raw
materials; PENRT = Total use of non-renewable primary energy resources; SM = Use of secondary material; RSF = Use of renewable secondary fuels;
NRSF = Use of non-renewable secondary fuels; FW = Use of net fresh water
RESULTS OF THE LCA – WASTE CATEGORIES AND OUTPUT FLOWS according to EN 15804+A2:
1 m^2 Fabric Tapes
Parameter Unit A1-A3 A4 A5 C1 C2 C3 D
HWD kg 5.11E-05 7.32E-13 2.61E-12 0 2.41E-14 4.72E-12 -1.17E-10
NHWD kg 4.91E-02 2.85E-05 1.78E-02 0 9.39E-07 3.8E-02 -1.04E-03
RWD kg 3.75E-04 2.56E-07 3.51E-06 0 8.43E-09 5.85E-06 -1.61E-04
CRU kg 0 0 0 0 0 0 0
MFR kg 0 0 0 0 0 0 0
MER kg 0 0 0 0 0 0 0
EEE MJ 0 0 2.26E-01 0 0 3.09E-01 0
EET MJ 0 0 4.19E-01 0 0 5.79E-01 0
HWD = Hazardous waste disposed; NHWD = Non-hazardous waste disposed; RWD = Radioactive waste disposed; CRU = Components for re-use;
MFR = Materials for recycling; MER = Materials for energy recovery; EEE = Exported electrical energy; EET = Exported thermal energy
6 Environmental Product Declaration - Sifloor AG - Fabric Tape
RESULTS OF THE LCA – additional impact categories according to EN 15804+A2-optional:
1 m^2 Fabric Tapes
Parameter Unit A1-A3 A4 A5 C1 C2 C3 D
Disease
PM ND ND ND ND ND ND ND
incidence
IR kBq U235 eq ND ND ND ND ND ND ND
ETP-fw CTUe ND ND ND ND ND ND ND
HTP-c CTUh ND ND ND ND ND ND ND
HTP-nc CTUh ND ND ND ND ND ND ND
SQP SQP ND ND ND ND ND ND ND
PM = Potential incidence of disease due to PM emissions; IR = Potential Human exposure efficiency relative to U235; ETP-fw = Potential comparative
Toxic Unit for ecosystems; HTP-c = Potential comparative Toxic Unit for humans (cancerogenic); HTP-nc = Potential comparative Toxic Unit for humans
(not cancerogenic); SQP = Potential soil quality index
Disclaimer 1 – for the indicator 'Potential Human exposure efficiency relative to U235'. This impact category deals mainly with the
eventual impact of low-dose ionizing radiation on human health of the nuclear fuel cycle. It does not consider effects due to possible
nuclear accidents, occupational exposure or radioactive waste disposal in underground facilities. Potential ionizing radiation from the
soil, radon and from some construction materials is also not measured by this indicator.
Disclaimer 2 – for the indicators 'abiotic depletion potential for non-fossil resources', 'abiotic depletion potential for fossil resources',
'water (user) deprivation potential, deprivation-weighted water consumption', 'potential comparative toxic unit for ecosystems', 'potential
comparative toxic unit for humans – cancerogenic', 'Potential comparative toxic unit for humans - not cancerogenic', 'potential soil
quality index'. The results of this environmental impact indicator shall be used with care as the uncertainties on these results are high
as there is limited experience with the indicator.
Disclaimer 3: Additional environmental impact indicators (EN 15804, Table 4) are not declared in the EPD. The results of these
environmental impact indicators should be used with caution as the uncertainties in these results are high and there is limited
experience with the indicators (see ILCD classification in EN 15804, Table 5). For this reason, the results based on these indicators are
not reported.
6. LCA: Interpretation
for in Module A5 in the form of biogenic CO emissions.
2
The coefficient of variation is a measure of the relative scatter.
It indicates what percentage of the average the standard
deviation is. It is therefore the percentage ratio of the standard
deviation to the arithmetic mean. It is used to make it easier to
compare the spread of different distributions. The spread of the
impact indicators is generally low and at about the same level
for all indicators.
Alongside the coefficient of variation, the maximum deviation of
individual products' impact from the average value for specific
impact indicators was also analysed (see table below). These
show that some impact indicators such as Ozone Depletion
react sensitively to individual substances contained, resulting in
a high deviation. In general, however, the results are in the
same order of magnitude, which indicates a appropriate
grouping.
The dominance analysis of the impact assessment indicators
shows a large contribution from the manufacturing phase (A1-
A3). A large proportion of the environmental impact stems from
the raw materials used (A1), with the synthetic polymer
dispersions making the highest contributions (with regard to the
impact indicator Climate Change - total, an average of 90% of
the impact in A1 is attributable to this component).
In addition, the waste treatment of the packaging and the
product (A5, C3) plays a major role for the Climate Change -
total impact assessment indicator. In these modules, thermal
utilisation was modelled as a worst-case scenario. The large
proportion in module A5 in particular can be explained by the
fact that in addition to the waste treatment of the packaging, the
waste treatment of the protective paper is also declared in this
module, which on average accounts for one fourth of the total
mass of the product. Furthermore, both the packaging and the
protective paper contain biogenic carbon, which is accounted
7 Environmental Product Declaration - Sifloor AG - Fabric Tape
renewable energy resources contained in the raw materials and
packaging materials with biogenic content.
The coefficients of variation of the life cycle inventory indicators
generally show a low level of scatter. Among the life cycle
inventory indicators, the results for the indicators Hazardous
waste disposed, Non-hazardous waste disposed (NHWD) and
Radioactive waste disposed (RWD) show the highest scatter,
which is due to differences in the product formulations
considered.
The assumptions used to determine the reported impact
indicator results are presented in Chapter 3.3. Specific data
was used for operational activities in phases A2-A3. Raw
material inputs (A1) were mainly modelled using generic
background data sets. Raw material inputs in particular have a
major influence on all the indicators shown, so care was taken
here to use data sets that are representative in terms of
technological aspects. In order to achieve this, also data sets
were used whose reference year was up to 10 years in the
In relation to the life cycle inventory indicators Total use of past, which led to an overall medium temporal
renewable primary energy resources (PERT) and Total use of representativeness. With regard to geographical aspects, the
non-renewable primary energy resources (PENRT), the largest results presented in this EPD are representative for Europe.
share of energy consumption in the life cycle occurs in the Activities in the downstream life cycle phases (A4-A5; C1-C3)
manufacturing phase (A1-A3). Significant contributions to were modelled using scenarios, whereby assumptions were
primary energy demand - non-renewable (PENRT) come from made regarding transport distance, for example. However,
the energy resources contained in the raw materials. The these life cycle phases are not dominant for the reported impact
largest contribution to primary energy demand - renewable indicators.
(PERT) is the consumption of renewable energy resources
needed to generate and provide electricity, as well as the
7. Requisite evidence
Technical data sheet, Safety Data Sheet, license of EMICODE according to ISO 16000-11 in a test chamber. Testing for
EC1 PLUS, certificate of the German Blue Angel and other carcinogenic, mutagenic, reprotoxic (CMR) substances and
product-related information are available for download at TVOC/TSVOC after 3 and 28 days.
https://int.uzin.com 7.1 VOC emissions Furthermore, the emission of volatile organic compounds from
building products in accordance with the award criteria for the
TVOC* limit values EMICODE following the AgBB scheme
eco-label "Low-emission floor covering adhesives and other
for EMICODE EC1 Plus (28 days [µg/m³])
flooring installation materials, DE-UZ 113', were determined.
Name Value Unit
TVOC (C6 - C16) ≤ 60 μg/m3 Date of test report: Test report dated 24 February 2022;
Sum SVOC (C16 - C22) ≤ 40 μg/m3
Result: The product complies with the requirements according
R (dimensionless) ≤ 1 -
to the GEV test method for 'EMICODE EC 1 PLUS – very low
VOC without NIK ≤ 40 μg/m3
emissions' classification and fulfils the requirements according
Carcinogenic Substances ≤ 1 μg/m3 to the award basis for DE-UZ 113.
TVOC* limit values BLUE ANGEL DE-UZ 113 following the AgBB scheme
AgBB scheme (28 days [µg/m³]) The requirements on emission performance according to AgBB
Name Value Unit for the ü-mark are automatically regarded as satisfied for
TVOC (C6 - C16) Specific products availing of EMICODE EC 1 PLUS classification.
≤ 60 μg/m3
concentration
Sum SVOC (C16 - C22) Specific
≤ 50 μg/m3
concentration
R (dimensionless) ≤ 1
VOC without LCI Specific concentration ≤ 40 μg/m3
Carcinogenic Substances Specific ≤ 1 per single
μg/m3
concentration value
Acetic acid ≤ 140 μg/m3
Formaldehyde ≤ 0.05 ppm
Other aldehydes ≤ 0.05 ppm
Test institute: WESSLING GmbH, Germany, 48341 Altenberge
Measuring process: GEV test method for determining the
emissions of volatile organic compounds from building products
8 Environmental Product Declaration - Sifloor AG - Fabric Tape
8. References
Standards: BREEAM
BREEAM (Building Research Establishment Environmental
DIN 18356 Assessment Methodology);
DIN 18356: German construction contract procedures (VOB) - https://bregroup.com/products/breeam [2023]
Part C: General technical specifications in construction
contracts (ATV) - Laying of parquet flooring and wood block Candidate list
flooring. List of substances of very high concern for Authorisation,
published in accordance with Article 59(10) of the REACH
EN 13501-1 Regulation, ECHA, www.echa.europa.eu/candidate-list-table
DIN EN 13501-1:2019, Fire classification of construction [2023]
products and building elements - Part 1: Classification using
data from reaction to fire tests. DGNB
DGNB – German Sustainable Building Council; www.dgnb.de
EN 15804 [2023]
EN 15804:2012+A2:2019+AC:2021, Sustainability of
construction works — Environmental Product Declarations — EMICODE
Core rules for the product category of construction products. GEV (Gemeinschaft Emissionskontrollierte Verlegewerkstoffe,
Klebstoffe und Bauprodukte e.V. Düsseldorf);
ISO 14025 www.emicode.com/en [2023]
EN ISO 14025:2011, Environmental labels and declarations —
Type III environmental declarations — Principles and EWC
procedures. European Waste Catalog established by Commission decision
2000/532/EC. http://www.environment-agency.gov.uk/ [2023]
ISO 14040
DIN EN ISO 14040: 2006, Environmental management – Life German AgBB
cycle assessment – Principles and framework (ISO Committee for Health-related Evaluation of Building Products:
14040:2006); German and English versions EN ISO health-related evaluation of emissions of volatile organic
14040:2006. compounds (VOC and SVOC) from building products;
www.umweltbundesamt.de/produkte/bauprodukte/agb b.htm
ISO 14044 [2012]
DIN EN ISO 14044: 2006, Environmental management – Life
cycle assessment – Requirements and guidelines (ISO IBU 2021
14044:2006); German and English versions EN ISO Institut Bauen und Umwelt e.V.: General Instructions for the
14044:2006. EPD programme of Institut Bauen und Umwelt e.V., Version
2.0, Berlin: Institut Bauen und Umwelt e.V., www.ibu-epd.com
ISO 15686 [2023]
DIN ISO 15686:2017, Buildings and constructed assets --
Service life planning. DIN EN 13501. LCA For Experts Software
LCA For Experts Software system (Version 10) and Database
ISO 16000-11 for Life Cycle Engeneering (Content Version 2023.2). Sphera
DIN EN ISO 16000-11:2006-06, Indoor air – Part 11: Solutions GmbH, Leinfelden-Echterdingen [2023]
Determination of the emission of volatile organic compounds
from building products and furnishings – Sampling, storage of LEED
samples and preparation of test specimens. LEED (Leadership in Energy and Environmental Design);
https://worldgbc.org/ [2023]
ISO 22633
DIN EN ISO 22632:2019, Adhesives - Test methods for Ordinance on Biocide Products No. 528/2012
adhesives for floor coverings and wall coverings - Regulation (EU) No 528/2012 of the European Parliament and
Determination of dimensional changes of a linoleum floor of the Council of 22 May 2012 concerning the making available
covering in contact with an adhesive. on the market and use of biocidal products[2012]
ISO 22635 PCR Part A
Adhesives - Test method for adhesives for plastic or rubber Product Category Rules for Building-Related Products and
floor coverings or wall coverings - Determination of dimensional Services, Part A: Calculation Rules for the Life Cycle
changes after accelerated ageing. Further References: Assessment and Requirements on the Project report, Version
1.3, Institut Bauen und Umwelt e.V. [08/2022]
Blue Angel (DE-UZ 113)
Bundesministerium für Umwelt, Naturschutz und PCR Part B
Reaktorsicherheit, Umweltbundesamt, DE Deutsches Institut für Product Category Rules for Construction Products. Part B:
Gütesicherung und Kennzeichnung e.V.; Jury Ecolabel; Dispersion adhesives and primers for floor coverings, Version
https://www.blauer-engel.de/en [2023] 3, [06/2023]
BNB REACH
Assessment System for Sustainable Building; https://www.bnb- Directive (EG) No. 1907/2006 of the European Parliament and
nachhaltigesbauen.de/en/assessment-system/ [2023] of the Council dated 18 December 2006 on the registration,
evaluation, approval and restriction of chemical substances
(REACH), for establishing a European Agency for chemical
9 Environmental Product Declaration - Sifloor AG - Fabric Tape
substances, for amending Directive 1999/45/EC and for [2006]
annulment of Directive (EEC) No. 793/93 of the Council,
Directive (EC) No. 1488/94 of the Commission, Guideline Ü-mark
76/769/EEC of the Council and Guidelines 91/155/EEC, Ü-mark-Übereinstimmungszeichen; https://www.dibt.de/de
93/67/EEC, 93/105/EC and 2000/21/EC of the Commission. [2023]
10 Environmental Product Declaration - Sifloor AG - Fabric Tape
Publisher
Institut Bauen und Umwelt e.V. +49 (0)30 3087748- 0
Hegelplatz 1 info@ibu-epd.com
10117 Berlin www.ibu-epd.com
Germany
Programme holder
Institut Bauen und Umwelt e.V. +49 (0)30 3087748- 0
Hegelplatz 1 info@ibu-epd.com
10117 Berlin www.ibu-epd.com
Germany
Author of the Life Cycle Assessment
Uzin Utz SE 0731 4097 0
Dieselstraße 3 nachhaltigkeit@uzin-utz.com
89079 Ulm www.uzin-utz.de
Germany
Owner of the Declaration
Uzin Utz SE 0731 4097 0
Dieselstraße 3 nachhaltigkeit@uzin-utz.com
89079 Ulm www.uzin-utz.de
Germany
11 Environmental Product Declaration - Sifloor AG - Fabric Tape
