ENVIRONMENTAL PRODUCT DECLARATION
as per ISO 14025 and EN 15804+A2
Owner of the Declaration Kvadrat Acoustics A/S
Publisher Institut Bauen und Umwelt e.V. (IBU)
Programme holder Institut Bauen und Umwelt e.V. (IBU)
Declaration number EPD-KVC-20230217-CBC1-EN
Issue date 13.07.2023
Valid to 12.07.2028
Soft Cells Tracks 25mm (aluminium frame)
Kvadrat Acoustics
www.ibu-epd.com | https://epd-online.com
General Information
Kvadrat Acoustics Soft Cells Tracks 25mm (aluminium frame)
Programme holder Owner of the declaration
IBU – Institut Bauen und Umwelt e.V. Kvadrat Acoustics A/S
Hegelplatz 1 Orient Plads 1, 1
10117 Berlin 2150 Nordhavn
Germany Denmark
Declaration number Declared product / declared unit
EPD-KVC-20230217-CBC1-EN 1m2 configurable acoustic frame system
This declaration is based on the product category rules: Scope:
Textile covered acoustic frame systems, 01.08.2021 The declaration covers the average product Soft Cells Tracks 25mm (SC
(PCR checked and approved by the SVR) Tracks 25mm) with an aluminium frame and the Trevira CS textile. The SC
Tracks 25mm is a configurable textile-covered acoustic frame systems
from the company Kvadrat Acoustics. It is available with an aluminium
Issue date frame in customized sizes ranging from from 1000 mm x 500 mm x 25 mm
to 6000 mm x 3000 mm x 25 mm (L x W x H) and textile options under the
13.07.2023
textile series Trevira CS. The product is declared as a kit since it is
available by a single manufacturer as a set of multiple separate
components, which are assembled at the building site. All products
Valid to
included in this average EPD are produced in Kvadrat Acoustics
12.07.2028 production site, in Poland, and distributed to markets in France, Germany,
the United Kingdom and Spain. The products' components (including the
Trevira CS textile) are manufactured by Kvadrat Acoustics suppliers
located in Europe (Poland, Italy, Germany, Czech Republic). Production
data were collected for the period 2021-2022.
The owner of the declaration shall be liable for the underlying information
and evidence; the IBU shall not be liable with respect to manufacturer
information, life cycle assessment data and evidences.
The EPD was created according to the specifications of EN 15804+A2. In
the following, the standard will be simplified as EN 15804.
Dipl.-Ing. Hans Peters
Verification
(Chairman of Institut Bauen und Umwelt e.V.)
The standard EN 15804 serves as the core PCR
Independent verification of the declaration and data according to ISO
14025:2011
internally X externally
Florian Pronold Dr.-Ing. Nikolay Minkov,
(Managing Director Institut Bauen und Umwelt e.V.) (Independent verifier)
1 Environmental Product Declaration - Kvadrat Acoustics - Soft Cells Tracks 25mm (aluminium frame)
Product
Performance data of the product with respect to its
Product description/Product definition characteristics in accordance with the relevant technical
SC Tracks 25 mm with aluminium profile and Trevira CS textile provision (no CE-making).
is a site-fabricated acoustical wall system, which stretches
textile over semi-rigid acoustic padding to control sound and Base materials/Ancillary materials
add to the aesthetic design of interior spaces. The product is The constituents of the product are shown in the table below.
available in customized sizes and different textile options under Packaging and installation materials are not included. The SC
the trade name Soft Cells Tracks 25mm. This EPD includes Tracks 25 mm system consists of an aluminium frame,
only the Soft Cells Tracks with aluminium frame and Trevira CS aluminium corners, a tensioning mechanism (leaf spring), a
textile option. The product is declared as a construction product cone spring for retaining the absorber, a layer of mineral glass
'kit', since it consists of multiple separate components and wool absorber, and Trevira CS textile (polyester textile) for the
placed on the market by a single manufacturer. The system panel's wear. Installation screws are required to install the
consists of a single-sided layer of tensioned textile, attached to system however, these are not part of the product order and
an aluminium frame profile, over a mineral-based acoustic core, are purchased separately from the installers at the building site
with an integrated tension system. (installation material). The amount of installation screws is 0.14
kg/m2 of SC Tracks 25 mm. The SC Tracks 25 mm packaging
For the use and application of the product the respective includes core board and low density polyethylene (LD PE) film
national provisions at the place of use apply, in Germany for packaging for the Trevira CS textile roll.
example the Building Codes of the federal states and the
corresponding national specifications. This product does not contain substances listed in the
candidate list (date: 25.06.2020) exceeding 0.1 percentage by
Application
mass.
SC Tracks 25mm controls sound and add to the aesthetic
design of interior spaces. The system is intended for interior
Name Value Unit
walls and is particularly well suited for spaces with severe to
Aluminium frame (profile) 17.44 wt-%
moderate need for sound absorption, large free wall surfaces,
and late changes as the tracks are built on-site. It is installed Tensioning mechanism (steel leaf spring) 4.74 wt-%
directly on wall substrate and can be applied in many different Aluminium corner 0.76 wt-%
markets, architectural needs and acoustic environments. Retaining cone spring (steel cone spring) 0.73 wt-%
Technical Data Sound absorber (mineral glass wool) 67.14 wt-%
The product has a sound adsorption class B to D according to Trevira CS textile (polyester textile) 9.19 wt-%
ISO 11654 with a sound absorption coefficient of 0.55-0.85
(ISO 354). The fire performance is B-s2,d0 and C-s2,d0. The Manufacturing and assembly
dimensions of the system after its installation in the building site All components are manufactured by Kvadrat Acoustics
are: suppliers, located in Europe. The components are delivered to
Kvadrat Acoustics production site in Poland, where they are
Typical size panel: 2600 mm x 1300 mm x 25 mm stored temporarily and processed before being transported to
Min. size panel: 1000 mm x 500 mm x 25 mm warehouses in France, Germany, the United Kingdom, and
Max. size panel: 6000 mm x 3000 mm x 25 mm Spain. The Trevira CS textile is shipped from the supplier to the
warehouses directly. Upon their arrival at the warehouses, the
The components comprising the product kit are delivered at the components are stored and assembled into a kit and then
building site with the following dimensions. The components shipped to the building site.
arrive at the building site in fixed dimensions however, the
number of component pieces differs across systems with
different sizes.
Aluminium frame (2 profiles): 25.9 mm x 25 mm x 3000 mm
Aluminium corner: 35 mm x 35 mm x 25 mm
Tensioning mechanism (leaf spring): 7 mm x 14 mm x 1000 mm
Mineral glass wool absorber: 1200 mm x 1200 mm x 22 mm
Retaining cone spring: 6 mm x 6 mm x 2 mm
Trevira CS textile (roll): 400 mm x 400 mm x 1500 mm
Constructional data
Name Value Unit
Sound adsorption class cf. ISO
B to D
11654
Sound absorption coefficient cf. ISO-
0.55 - 0.85 -
354
Dimensions max. (L x W x H) 6000x3000x25 mm
Dimensions min. (L x W x H) * 1000x500x25 mm
B-s2,d0 and C-
Fire performance cf. EN-13501-1 -
s2,d0
* Smaller sizes are available from Kvadrat Acoustics, but are
not covered by the EPD.
2 Environmental Product Declaration - Kvadrat Acoustics - Soft Cells Tracks 25mm (aluminium frame)
SC Tracks 25 mm is assembled and installed at the building
site (France, Germany, United Kingdom, Spain). This procedure
includes cutting the frame profiles, absorber, and Trevira CS
textile to the required size and installing the panel. Most of
these activities are done manually without any materials
consumption. An electric sawn and screwdriver are used. After
the building or the product reaches its end-of-life stage, the
system is removed and dismantled. This process requires
mostly manual work.
Reference service life
The RSL is 50 years.
LCA: Calculation rules
were collected.
Declared Unit
The declared unit is 1m2 configurable acoustic frame system. System boundary
All SC Tracks 25mm sizes, included in this EPD, consist of the The EPD is of the type cradle-to-gate with options, modules A4,
same type of components and no variation takes place A5, C1-C4 and D. The product stage (A1-A3) includes:
regarding the components' type. The amount of each A1 - Raw material extraction, processing, processing of
component per declared unit differs between different product secondary material input (e.g. recycling processes) and
sizes. No component was included as an unweighted average. production of the components. The production of excess
The results correspond to a typical SC Tracks 25 mm size of components to compensate for material losses during the
1300 mm x 2600 mm x 25 mm (LxWxH), which represents all installation phase, as well as the production of ancillary
the product sizes included in this EPD. Finally, this EPD covers materials (installation screws), are accounted for in module A1
only the Trevira CS textile option, which is a polyester textile. because the product is declared as a kit.
A2 - Transport of components and packaging from the suppliers
Declared unit
to Kvadrat Acoustics production site, as well as internal
The declared unit is 1m2 configurable acoustic frame system
transport of components from the production site to
with a conversion factor of 3.11 kg/m2. warehouses.A3 - Assembly of components into a product kit.
Name Value Unit The production of sales packaging (plastic and core board
Declared unit 1 m2 packaging for the textile) is included in module A3.
Grammage 3.11 kg/m2
The construction process stage (A4-A5) includes:
Content of frame (based on weight) 17.44 % A4 - Transport of the kit from Kvadrat Acoustics warehouses to
Content of textile membrane (based on weight) 9.19 % the building site. Module A4 includes also the transport of
Content of in-fill (based on weight) 67.14 % ancillary materials (installation screws) from the supplier to the
building site (the product is declared as a kit).
Deviation from frame (max. kg/m²)* 145 %
A5 - Installation of SC Tracks 25mm system at the application
Panel size typical 3.38 m2
site including in-situ processing of components (cutting the
Layer thickness 0.025 m components to the correct size). Module A5 also includes the
transport and processing of waste (material loss, packaging)
* The maximum percentage deviation of the frame refers to the
generated in the application site.
minimum size (500 mm x 1000 mm x 25 mm). For the
maximum size (1300 mm x 2600 mm x 25 mm) the deviation
The end-of-life stage includes:
is -56 %.
C1 - Deconstruction and dismantling of the system. The manual
dismantling impact of the system is considered negligible and
The LCA values included in this EPD are considered robust.
module C1 is reported without any impacts.
The reference product groups considered in this EPD are
C2 - Transport of waste from the building site to Material
assembled into kits in the same production and storing facilities,
Recovery Facilities (MRF), as well as transport of recyclable
while the components are manufactured by the same suppliers.
and non-recyclable waste from MRF to recycling facilities and
In addition, the background datasets used are representative of
landfill, respectively.
the geographical scope, technologies and production
C3 - Waste processing for dismantling the system into
processes used. Therefore, variations in geography are not
components and sorting the components/materials to waste for
relevant. Plant production data for the period of 2021-2022
material recovery and landfill.
3 Environmental Product Declaration - Kvadrat Acoustics - Soft Cells Tracks 25mm (aluminium frame)
C4 - Disposal of non-recyclable components/materials (textile, into account.
absorber) to landfill.
Module D includes reuse, recovery and/or recycling potentials. Data Quality
Benefits originating from the recycling of material loss and Background data were retrieved from Managed LCA Content
metal components after reaching their end-of-life stage, as well database (formerly known as GaBi database) version 2022.2
as the incineration of plastic packaging, were considered in provided by Sphera. The quality of foreground and background
module D data is considered very good and all major processes are
represented with data of good quality in compliance with the
stated criteria from the PCR. In addition, the conservative
Geographic Representativeness approach was adopted when foreground data quality was
Land or region, in which the declared product system is insufficient. The background data are up to date and the
manufactured, used or handled at the end of the product´s temporal data quality requirements of the PCR are generally
lifespan: Europe met. The temporal span of the background data used ranges
from 2015 to 2026 and no data are more than 10 years old.
Allocation of energy used for storing, moving and assembling
Comparability
the product kit in module A3 was performed. The allocation key
Basically, a comparison or an evaluation of EPD data is only
is the area occupied by the SC Tracks 25 mm in the production
possible if all the data sets to be compared were created
site and warehouses since the activities are dependent on the
according to EN 15804 and the building context, respectively
product's area.
the product-specific characteristics of performance, are taken
LCA: Scenarios and additional technical information
Characteristic product properties of biogenic carbon
Reference service life
The SC Tracks 25 mm with the Trevira CS textile do not include
any materials with biogenic carbon content. The product's Name Value Unit
packaging includes biogenic carbon due to the presence of a Reference service life 50 years
core board in the Trevira CS textile packaging.
End of life (C1 - C4)
Information on describing the biogenic Carbon Content at
Name Value Unit
factory gate
Metal components (aluminium, steel) EoL %
Name Value Unit 100
scenario recycling
kg
Biogenic carbon content in product - Mineral glass wool absorber EoL scenario 100 % landfill
C
Trevira CS textile EoL scenario 100 % landfill
Biogenic carbon content in accompanying kg
packaging (core board) 0.00562 C Collected separately - kg
Collected as mixed construction waste * 3.25 kg
Technical scenario information for the declared modules A4, A5, Recycling ** 0.87 kg
C1-C4 and D is provided in the following tables. The electricity Landfilling 2.38 kg
consumption and material loss in module A5 were measured for
* The amount of output waste includes the installation screws.
the typical SC Tracks 25 mm size based on the actual activities
** The amount of waste to be recycled includes the installation
taking place during the system's installation at the building site.
screws.
An end-of-life (EoL) scenario was established for the packaging
waste in module A5 which assumes that the core board
Reuse, recovery and/or recycling potentials (D), relevant
packaging waste is recycled, while the plastic packaging waste
scenario information
is incinerated.
Name Value Unit
Transport to the building site (A4)
Replaced primary aluminium 0.13 kg
Name Value Unit
Replaced primary steel 0.15 kg
Litres of fuel 0.0221 l/100km
Replaced primary galvanized steel 0.14 kg
Transport distance 17.6 km
Replaced primary mineral glass wool 0.041 kg
Capacity utilisation (including empty runs) 51 %
Replaced electricity (grid mix) 7.82E-03 kWh
Gross density of products transported 124.52 kg/m3
Replaced thermal energy (natural gas) 5.01E-02 MJ
Installation into the building (A5)
Name Value Unit
Auxiliary (galvanised steel screws) 0.135 kg
Electricity consumption 0.00215 kWh
Material loss (frame, absorber, textile) 0.229 kg
Plastic packaging for incineration 4.21E-03 kg
Core board packaging for recycling 1.38E-02 kg
4 Environmental Product Declaration - Kvadrat Acoustics - Soft Cells Tracks 25mm (aluminium frame)
LCA: Results
DESCRIPTION OF THE SYSTEM BOUNDARY (X = INCLUDED IN LCA; ND = MODULE OR INDICATOR NOT DECLARED; MNR =
MODULE NOT RELEVANT)
Benefits and
Construction loads beyond
Product stage Use stage End-of-life stage
process stage the system
boundaries
la ire ta m w a Ry lp p u s tro p s n a rT g n iru tc a fu n a M e h t m o rf tro p s n a rTe tis e h t o t e ta g y lb m e s s A e s U e c n a n e tn ia M ria p e R tn e m e c a lp e R tn e m h s ib ru fe R y g re n e la n o ita re p Oe s u re ta w la n o ita re p Oe s u n o itc u rts n o c -e Dn o itilo m e d tro p s n a rT g n is s e c o rp e ts a W la s o p s iD -e s u e R-y re v o c e R-g n ilc y c e Rla itn e to p
A1 A2 A3 A4 A5 B1 B2 B3 B4 B5 B6 B7 C1 C2 C3 C4 D
X X X X X MND MND MNR MNR MNR MND MND X X X X X
RESULTS OF THE LCA - ENVIRONMENTAL IMPACT according to EN 15804+A2: 1 m² Soft Cells Tracks 25mm (aluminium
frame)
Parameter Unit A1 A2 A3 A4 A5 C1 C2 C3 C4 D
GWP-total kg CO 2 eq 1.11E+01 4.14E-01 1.87E-01 1.28E-02 6.85E-02 0 1.87E-01 8.7E-03 4.71E-01 -1.75E+00
GWP-fossil kg CO 2 eq 1.17E+01 4.1E-01 1.76E-01 1.27E-02 4.61E-02 0 1.86E-01 8.66E-03 6.95E-02 -1.75E+00
GWP-
biogenic kg CO 2 eq -5.53E-01 8.38E-04 1.05E-02 2.62E-05 2.22E-02 0 3.82E-04 1.48E-06 4.01E-01 9.83E-04
GWP-luluc kg CO 2 eq 2.9E-03 2.78E-03 4.95E-04 8.73E-05 2.06E-04 0 1.27E-03 4.01E-05 6.77E-05 -2.92E-04
ODP kg CFC11 eq 1.07E-08 4.07E-14 1.17E-09 1.27E-15 1.36E-10 0 1.85E-14 1.29E-14 1.01E-13 -2.82E-14
AP mol H+ eq 4.37E-02 5E-04 3.17E-04 1.46E-05 4.72E-05 0 2.69E-04 4.47E-05 3.25E-04 -6.14E-03
EP-
kg P eq 5.01E-05 1.48E-06 6.66E-06 4.63E-08 2.28E-07 0 6.75E-07 2.49E-08 3.93E-06 -6.83E-07
freshwater
EP-marine kg N eq 8.58E-03 1.68E-04 1.09E-04 4.69E-06 1.88E-05 0 9.8E-05 2.04E-05 2.59E-04 -1.1E-03
EP-terrestrial mol N eq 1.44E-01 1.99E-03 1.09E-03 5.66E-05 2.19E-04 0 1.14E-03 2.26E-04 9.95E-04 -1.3E-02
kg NMVOC
POCP 2.03E-02 4.52E-04 2.52E-04 1.25E-05 4.6E-05 0 2.4E-04 5.56E-05 3.94E-04 -3.33E-03
eq
ADPE kg Sb eq 7.02E-06 4.17E-08 1.17E-07 1.31E-09 8.66E-09 0 1.9E-08 9.61E-09 4.62E-09 -7.46E-08
ADPF MJ 1.86E+02 5.45E+00 4.97E+00 1.7E-01 3.94E-01 0 2.48E+00 1.69E-01 6.98E-01 -2.01E+01
m3 world eq
WDP 1.29E+00 4.62E-03 3.45E-02 1.45E-04 2.11E-03 0 2.11E-03 1.67E-03 4.96E-03 -6.66E-02
deprived
GWP = Global warming potential; ODP = Depletion potential of the stratospheric ozone layer; AP = Acidification potential of land and water; EP =
Eutrophication potential; POCP = Formation potential of tropospheric ozone photochemical oxidants; ADPE = Abiotic depletion potential for non-fossil
resources; ADPF = Abiotic depletion potential for fossil resources; WDP = Water (user) deprivation potential)
RESULTS OF THE LCA - INDICATORS TO DESCRIBE RESOURCE USE according to EN 15804+A2: 1 m² Soft Cells Tracks
25mm (aluminium frame)
Parameter Unit A1 A2 A3 A4 A5 C1 C2 C3 C4 D
PERE MJ 4.91E+01 3.76E-01 4.92E-01 1.18E-02 2.08E-02 0 1.72E-01 1.36E-02 8.52E-02 -4.66E+00
PERM MJ 4.26E+00 0 1.68E-01 0 0 0 0 0 0 0
PERT MJ 5.34E+01 3.76E-01 6.6E-01 1.18E-02 2.08E-02 0 1.72E-01 1.36E-02 8.52E-02 -4.66E+00
PENRE MJ 1.78E+02 5.47E+00 4.79E+00 1.71E-01 5.79E-01 0 2.49E+00 1.7E-01 6.98E-01 -2.02E+01
PENRM MJ 7.4E+00 0 1.83E-01 0 -1.83E-01 0 0 0 0 0
PENRT MJ 1.86E+02 5.47E+00 4.97E+00 1.71E-01 3.96E-01 0 2.49E+00 1.7E-01 6.98E-01 -2.02E+01
SM kg 1.75E+00 0 1.38E-02 0 0 0 0 0 0 0
RSF MJ 0 0 0 0 0 0 0 0 0 0
NRSF MJ 0 0 0 0 0 0 0 0 0 0
FW m3 6.18E-02 4.34E-04 1.51E-03 1.36E-05 6.44E-05 0 1.98E-04 4.74E-05 1.48E-04 -1.08E-02
PERE = Use of renewable primary energy excluding renewable primary energy resources used as raw materials; PERM = Use of renewable primary
energy resources used as raw materials; PERT = Total use of renewable primary energy resources; PENRE = Use of non-renewable primary energy
excluding non-renewable primary energy resources used as raw materials; PENRM = Use of non-renewable primary energy resources used as raw
materials; PENRT = Total use of non-renewable primary energy resources; SM = Use of secondary material; RSF = Use of renewable secondary fuels;
NRSF = Use of non-renewable secondary fuels; FW = Use of net fresh water
RESULTS OF THE LCA – WASTE CATEGORIES AND OUTPUT FLOWS according to EN 15804+A2:
1 m² Soft Cells Tracks 25mm (aluminium frame)
Parameter Unit A1 A2 A3 A4 A5 C1 C2 C3 C4 D
HWD kg 2.4E-08 2.89E-11 2.41E-10 9.03E-13 -1.23E-12 0 1.32E-11 2.12E-12 6.55E-11 -6.1E-10
NHWD kg 8.19E-01 8.89E-04 7.59E-04 2.78E-05 1.86E-04 0 4.05E-04 4.5E-05 2.31E+00 -2.55E-01
RWD kg 7.38E-03 1.01E-05 9.55E-04 3.17E-07 9.01E-07 0 4.62E-06 2.24E-06 8.1E-06 -1.14E-03
CRU kg 0 0 0 0 0 0 0 0 0 0
MFR kg 0 0 3.38E-01 0 2.43E-01 0 0 8.72E-01 0 0
5 Environmental Product Declaration - Kvadrat Acoustics - Soft Cells Tracks 25mm (aluminium frame)
MER kg 0 0 0 0 4.21E-03 0 0 0 0 0
EEE MJ 0 0 0 0 2.82E-02 0 0 0 0 0
EET MJ 0 0 0 0 5.01E-02 0 0 0 0 0
HWD = Hazardous waste disposed; NHWD = Non-hazardous waste disposed; RWD = Radioactive waste disposed; CRU = Components for re-use;
MFR = Materials for recycling; MER = Materials for energy recovery; EEE = Exported electrical energy; EET = Exported thermal energy
RESULTS OF THE LCA – additional impact categories according to EN 15804+A2-optional:
1 m² Soft Cells Tracks 25mm (aluminium frame)
Parameter Unit A1 A2 A3 A4 A5 C1 C2 C3 C4 D
Disease
PM 4.4E-07 3.94E-09 3.13E-09 1E-10 3.37E-10 0 1.6E-09 8.48E-10 3.72E-09 -6.53E-08
incidence
IR kBq U235 eq 1.1E+00 1.53E-03 2.09E-01 4.79E-05 1.32E-05 0 6.98E-04 3.66E-04 1.03E-03 -2.53E-01
ETP-fw CTUe 4.37E+02 3.86E+00 2.4E+00 1.21E-01 3.05E-01 0 1.76E+00 1.13E-01 9.26E-01 -9.56E+00
HTP-c CTUh 6.51E-09 7.96E-11 4.06E-11 2.48E-12 5.15E-12 0 3.62E-11 2.43E-12 4.89E-11 -1.38E-09
HTP-nc CTUh 2.82E-07 4.31E-09 1.71E-09 1.34E-10 3.26E-10 0 1.97E-09 1.3E-10 5.42E-09 -1.51E-08
SQP SQP 9.89E+01 2.29E+00 8.64E-01 7.2E-02 1.71E-01 0 1.05E+00 3.83E-02 1.06E-01 -1.41E+00
PM = Potential incidence of disease due to PM emissions; IR = Potential Human exposure efficiency relative to U235; ETP-fw = Potential comparative
Toxic Unit for ecosystems; HTP-c = Potential comparative Toxic Unit for humans (cancerogenic); HTP-nc = Potential comparative Toxic Unit for humans
(not cancerogenic); SQP = Potential soil quality index
Disclaimer for the indicator 'potential Human exposure efficiency relative to U235': This impact category deals mainly with the eventual
impact of low dose ionizing radiation on human health of the nuclear fuel cycle. It does not consider effects due to possible nuclear
accidents, occupational exposure nor radioactive waste disposal in underground facilities. Potential ionizing radiation from the soil,
radon and from some construction materials is also not measured by this indicator.
Disclaimer for the indicators 'abiotic depletion potential for fossil resources', 'abiotic depletion potential for non-fossil resources', 'water
(user) deprivation potential', 'deprivation-weighted water consumption', 'potential comparative toxic unit for ecosystems', 'potential
comparative toxic unit for humans - cancer effects', 'potential comparative toxic unit for humans – non-cancer effects', 'potential soil
quality index': The results of this environmental impact indicator shall be used with care as the uncertainties on these results are high
or as there is limited experience with the indicator.
The major contributor across all environmental impact indicators (except GWP-biogenic) is module A1. This is expected since the SC
Tracks 25 mm is a product kit, the entire manufacturing of components takes place in Kvadrat Acoustics A/S upstream supply chain.
Module A1 has the lowest negative impact in the GWP-biogenic indicator due to the production of packaging (pallets, core board). In
addition, the activities taking place in Kvadrat Acoustics sites relate to the storing, moving and preparing of the product kit which does
not require high energy consumption. Therefore, module A3 has a low contribution to the environmental impacts. Finally, the use of
secondary material includes aluminium and steel (Module A1), as well as a core board (Module A3). The use of secondary fuels is
included in secondary datasets yet no secondary fuels are used in Kvadrat Acoustics sites.
References
ISO 11654 EN13501-1, 2018: Fire classification of construction products
ISO 11654, 1997: Acoustics — Sound absorbers for use in and building elements - Part 1: Classification using data from
buildings — Rating of sound absorption reaction to fire tests.
ISO 354 ISO 14025
ISO 354, 2013: Acoustics - Measurement of sound absorption DIN EN ISO 14025:2011-10, Environmental labels and
in a reverberation room. declarations — Type III environmental declarations —
Principles and procedures.
IBU PCR 2018, Part B
Requirements on the EPD for Textile covered acoustic frame EN 15804
systems. Version 1.0; 01-2018. EN 15804:2019+A2 (in press), Sustainability of construction
works — Environmental Product Declarations — Core rules for
IBU PCR 2019, Part A the product category of construction products.
The Product Category Rules for Building-Related Products and
Services, Part A: Calculation Rules for the Life Cycle ECHA Candidate List
Assessment and Requirements on the Project Report according List of substances of very high concern considered for approval
to EN 15804+A2:2019, Version 1.3. from Institut Bauen und (status 25.06.2020) according to Article 59
Umwelt e.V. (IBU); para. 10 of the REACH Regulation. European Chemicals
Agency
IBU 2021
Institut Bauen und Umwelt e.V.: General Instructions for the GaBi LCA software and database
EPD programme of Institut Bauen und Umwelt e.V. Version 2.0, The LCA modelling software is GaBi program version
Berlin: Institut Bauen und Umwelt e.V., 2021. www.ibu- 10.5.1.125 with corresponding databases from Sphera
epd.com. Solutions GmbH. Documentation
www.gabisoftware.com/support/gabi.
EN 13501-1
6 Environmental Product Declaration - Kvadrat Acoustics - Soft Cells Tracks 25mm (aluminium frame)
Publisher
Institut Bauen und Umwelt e.V. +49 (0)30 3087748- 0
Hegelplatz 1 info@ibu-epd.com
10117 Berlin www.ibu-epd.com
Germany
Programme holder
Institut Bauen und Umwelt e.V. +49 (0)30 3087748- 0
Hegelplatz 1 info@ibu-epd.com
10117 Berlin www.ibu-epd.com
Germany
Author of the Life Cycle Assessment
FORCE Technology +4543250856
Park Alle 345 chme@forcetechnology.com
2605 Brøndby www.forcetechnology.com
Denmark
Owner of the Declaration
Kvadrat Acoustics A/S +4589531866
Orient Plads 1, 1 kvadratacoustics@kvadrat.org
2150 Nordhavn www.kvadratacoustics.com
Denmark
7 Environmental Product Declaration - Kvadrat Acoustics - Soft Cells Tracks 25mm (aluminium frame)
