ENVIRONMENTAL-PRODUCT DECLARATION
as per ISO 14025 and EN 15804+A2
Owner of the Declaration Interface
Publisher Institut Bauen und Umwelt e.V. (IBU)
Programme holder Institut Bauen und Umwelt e.V. (IBU)
Declaration number EPD-INT-20220227-CBB1-EN
Issue date 17.02.2023
Valid to 16.02.2028
Continuously dyed tufted tiles, 100% rec PA 6, a CQuest Bio Sone
backing
Interface
www.ibu-epd.com | https://epd-online.com
General Information
Interface Continuously dyed tufted tiles, 100% rec PA 6, a
CQuest Bio Sone backing
Programme holder Owner of the declaration
IBU – Institut Bauen und Umwelt e.V. Interface Europe Manufacturing BV
Hegelplatz 1 Industrielaan 15
10117 Berlin 3925ZG Scherpenzeel
Germany Netherlands
Declaration number Declared product / declared unit
EPD-INT-20220227-CBB1-EN 1 m² continuous-dyed modular carpet tiles with Sone acoustic felt covered
CQuest Bio (CQB) heavy backing and a pile material of PA 6 with 100%
recycled content
This declaration is based on the product category rules: Scope:
Floor coverings, 08.03.2023 The manufacturer declaration applies to tufted, continuous-dyed carpet
(PCR checked and approved by the SVR) tiles with a Sone polyester felt covered CQuest Bio backing, a pile material
of 100% recycled PA 6 with a maximum total pile weight of 1215 g/m2. The
products are tufted in Hasselt, the Netherlands. Dyeing of the surface is
Issue date performed externally. The dyed carpets are back coated in Scherpenzeel.
17.02.2023 LCA results for products with a maximum total pile weight of 580 g/m2 can
be taken from the corresponding tables of the annexe. Specific data for
every product within the declared group of products in relation to its total
Valid to pile weight can be calculated by using equation 1 given in the annexe (see
annexe chapter: 'General Information on the annexe'). The declaration is
16.02.2028 only valid in conjunction with a valid GUT-PRODIS license of the product.
The owner of the declaration shall be liable for the underlying information
and evidence; the IBU shall not be liable with respect to manufacturer
information, life cycle assessment data and evidences.
The EPD was created according to the specifications of EN 15804+A2. In
the following, the standard will be simplified as EN 15804 bezeichnet.
Verification
The standard EN 15804 serves as the core PCR
Independent verification of the declaration and data according to ISO
Dipl.-Ing Hans Peters 14025:2011
(chairman of Institut Bauen und Umwelt e.V.)
internally X externally
Dr. Alexander Röder Prof. Dr. Birgit Grahl,
(Managing Director Institut Bauen und Umwelt e.V.) (Independent verifier)
1 Environmental-Product Declaration - Interface - Continuously dyed tufted tiles, 100% rec PA 6, a CQuest Bio Sone backing
Product
floor coverings - Essential characteristics.
Product description/Product definition Additional product properties in accordance with EN 1307 can
The declaration applies to tufted carpet tiles having a surface be found on the Product Information System PRODIS using the
pile of 100% recycled polyamide 6 with a maximum total pile PRODIS
weight of 1215 g/m2. Colouring of the surface is performed registration number of the product (www.pro-dis.info) or on the
using continuous dyeing. The backing of the carpet consists of manufacturer's technical information section.
a CQuest Bio heavy backing covered by a Sone acoustic
polyester felt with a recycled content of 98%. The total recycled Base materials/Ancillary materials
content of the carpet is 82%. Name Value Unit
CQuest Bio backing system Sone: Polyamide 6 28.4 %
Backing compound based on renewable wood resin, containing
Polyester 12.1 %
a recycled
Ethylene vinyl acetate (EVA) 4.5 %
filler, glass-fleece reinforcement and polyester covering fleece.
For the placing on the market of the specific product in the Wood resin 6.5 %
European Additives 1.6 %
Union/European Free Trade Association (EU/EFTA) (with the Limestone 42.6 %
exception of
Aluminiumhydroxide 3.8 %
Switzerland) Regulation (EU) No. 305/2011 Construction
Glass fiber 0.5 %
Product Regulation (CPR) applies. The product needs a
Declaration of Performance (DoP) taking into The specific product covered by the EPD contains substances
consideration EN 14041:2018-05, Resilient, textile and laminate listed in the ECHA candidate list (08.07.2021)
floor coverings - Essential characteristics, and the CE-marking. exceeding 0.1
The DoP of the product can be found on the percentage by mass: no
manufacturer's technical information section. For the This product contains other CMR substances in
application and categories 1A or 1B which are not on the candidate list
use of the product the respective national provisions apply. exceeding 0.1
percentage by mass: no
Application Biocide products were added to this
The use class of the specific product as defined in construction product or it has been treated with biocide
EN 1307 can be found in the Product Information System products (this
(PRODIS) using the PRODIS registration number of the then concerns a treated product as defined by the (EU)
product. Ordinance on
Biocide Products No. 528/2012): no
Technical Data
Aluminium hydroxide is used as fire retardant.
The performance data listed in the Declaration of Performance
(DoP) apply. Environment and health during use
Constructional data according to EN 1307
Reference service life
Name Value Unit
The
Product Form Modular carpet tiles, 50 cm x 50 cm - service life of textile floor coverings strongly depends on the
Type of correct
Continuous-dyed, tufted carpet -
manufacture installation taking into account the declared use classification
Polyamide 6 from 100% recycled and
Yarn type -
material the adherence to cleaning and maintenance instructions.
A calculation of the reference service life according to ISO
Total carpet
4356 g/m2 15686 is not possible.
weight
Alternatively, a reference service life of 15 years can be
Secondary CQuest Bio backing with acoustic
- assumed,
backing textile bottom Sone
during which the functional and visual quality is guaranteed (In
Performance data of the product in accordance with the accordance with the warranty of the manufacturer). The
declaration of technical service life can be
performance with respect to its essential characteristics significantly longer.
according to EN 14041: 2018-05, Resilient, textile and laminate
LCA: Calculation rules
Name Value Unit
Declared Unit
Declared unit 1 m2
The declared unit and the mass reference must be indicated in
the appropriate table as declared. If there are several units to Grammage 4.356 kg/m2
choose from, a suitable one must be selected. If averages are Total thickness 8.6 mm
declared across various products, the average breakdown must Gross density 507 kg/m3
be explained.
The declared unit refers to 1 m2 produced textile floor covering.
1m² of floor covering with specified construction/composition The output of module A5 'Assembly' is 1 m2 installed textile
parameters. The mass reference should be indicated. floor covering.
The thickness of specific products is independent from its total
2 Environmental-Product Declaration - Interface - Continuously dyed tufted tiles, 100% rec PA 6, a CQuest Bio Sone backing
weight. The layer thickness of the specific product covered by relevant due to known VOC decay curves of the product.
the EPD can be found on the Product Information System
PRODIS using the PRODIS B2 Maintenance:
registration number of the product (www.pro-dis.info) or on the Cleaning of the textile floor covering for a period of 1 year:
manufacturer's technical information section. Vacuum cleaning – electricity supply
Wet cleaning – electricity, water consumption, production of the
For IBU core EPDs (where clause 3.6 is part of the EPD): for cleaning agent, waste water treatment
average EPDs, an estimate of the robustness of the LCA The
values must be made, e.g. concerning variability of the declared values in this module have to be multiplied by the
production process, geographical representativeness and the assumed
influence of background data and preliminary products service life of the floor covering in the building in question.
compared to the environmental impacts caused by actual B3 - B5:
production. The modules are not relevant within the assumed reference
service life of 15 years.
System boundary
B6 - B7:
Type of EPD: Cradle-to-gate with options No energy and water input are required for the operation of the
System boundaries of modules A, B, C, D: carpet in the use stage. The modules do not cause any
Modules C3, C4 and D are indicated separately for three end- environmental impact.
of-life scenarios: C1 De-construction:
1 - landfill disposal The floor covering is de-constructed manually and no additional
2 - municipal waste incineration environmental impact is caused.
3 - recovery in a cement plant
A1-A3 Production: C2 Transport:
Energy Transport
supply and production of the basic material, processing of of the carpet waste to a landfill, to the municipal waste
secondary incineration
material, auxiliary material, transport of the material to the plant (MWI) or to the waste collection facility for recycling.
manufacturing site, emissions, waste water treatment,
packaging material C3 Waste processing:
and waste processing up to the landfill disposal of residual C3-1: Landfill disposal needs no waste processing.
waste C3-2: Impact from waste incineration (plant with R1 >
(except radioactive waste). Benefits for generated electricity 0.6), generated electricity and steam are listed in the result
and steam table as exported energy.
due to the incineration of production waste are aggregated. C3-3:
Biogenic carbon that is stored in renewable material Collection of the carpet waste for recovery in the cement
(wood resin, renewable additives,packaging paper) is taken into industry,
account as well as the associated carbon dioxide waste processing (granulating), transport to the cement plant,
uptake from the air from which this biogenic carbon comes. emissions
from the incineration.
A4 Transport:
Transport of the packed textile floor covering from factory gate C4 Disposal
to the place of installation. C4-1: Impact from landfill disposal,
C4-2: The carpet waste leaves the system in module C3-2,
A5 Installation: C4-3: The pre-processed carpet waste leaves the system in
Installation module C3-3.
of the textile floor covering, processing of installation waste and
packaging waste up to the landfill disposal of residual waste D Recycling potential:
(except Calculated benefits result from materials exclusive secondary
radioactive waste), the production of the amount of carpet that materials (net materials).
occurs D-A5: Benefits for generated energy due to incineration of
as installation waste including its transport to the place of packaging and installation waste (incineration plant with R1 >
installation. 0.6),
Generated electricity and steam due to the incineration of D-1: Assuming that the chemically bound renewable
waste are listed in the result table as exported energy. materials in a landfill gas do not release landfill gas within 100
Biogenic carbon that is stored in renewable materials in years, no benefits due to landfill dosposal of carpet waste at the
installation waste and packaging paper is end-of-life are taken into account,
released as carbon dioxide emissions into the air at the end of D-2: Benefits for generated energy due to incineration of carpet
life in waste at the end-of-life (incineration plant with R1 > 0.6),
module A5. D-3: Benefits for saved fossil energy and saved inorganic
Preparation material due to recovery of the carpet in a cement plant.
of the floor and auxiliary materials (adhesives, fixing agents,
PET Geographic Representativeness
connectors) are beyond the system boundaries and not taken Land or region, in which the declared product system is
into account. manufactured, used or handled at the end of the product´s
B1 Use: lifespan: Europe
Indoor
emissions during the use stage. After the first year, no
product-related Volatile Organic Compound (VOC) emissions Comparability
are
3 Environmental-Product Declaration - Interface - Continuously dyed tufted tiles, 100% rec PA 6, a CQuest Bio Sone backing
Basically, a comparison or an evaluation of EPD data is only the product-specific characteristics of performance, are taken
possible if all the data sets to be compared were created into account.
according to EN 15804 and the building context, respectively
LCA: Scenarios and additional technical information
Characteristic product properties life
Information on biogenic carbon recommended by the manufacturer and the anticipated strain
on the floor
The biogenic carbon content quantifies the amount of biogenic by customers, the case-specific useful life can be established.
carbon in a construction product leaving the factory gate, and it Based on this useful
shall be separately declared for the product and for any life the
accompanying packaging. effects of module B2 need to be calculated in order to obtain
If the total mass of biogenic carbon containing materials is less the overall environmental impacts.
than 5 % of the total mass of the product and accompanying
Name Value Unit
packaging, the declaration of biogenic carbon content may be
Maintenance cycle (vacuum cleaning) 208 Number /year
omitted. The mass of packaging containing biogenic carbon
Maintenance cycle (wet cleaning) 1,5 Number /year
shall always be declared.
Water consumption (wet cleaning) 0.004 m3
Note: 1 kg of biogenic carbon is equivalent to 44/12 kg of CO2. Cleaning agent (wet cleaning) 0.09 kg
Electricity consumption 0.314 kWh
Name ValueUnit
For further information on cleaning and maintenance see
kg
Biogenic carbon content in product at factory gate 0.26 www.interface.com
C
Biogenic carbon content in accompanying kg
0.05
packaging at factory gate C
In case a reference service life according to applicable ISO
1 kg biogenic Carbon is equivalent to 44/12 kg of CO standards is declared then the assumptions and in-use
2
conditions underlying the determined RSL shall be declared. In
addition, it shall be stated that the RSL applies for the reference
The following technical scenario information is required for the conditions only.
declared modules and optional for non-declared modules.
The same holds for a service life declared by the manufacturer.
Modules for which no information is declared can be deleted;
Corresponding information related to in-use conditions needs
additional information can also be listed if necessary.
not be provided if a service life taken from the list on service life
The following technical information is a basis for the declared by BNB is declared.
modules or can be used for developing specific scenarios in the
context of a building assessment if modules are not declared Service life
(MND).
Name Value Unit
Life Span (according to
A5 is not declared including the disposal of the packaging 15 a
manufacturer's warranty)
material on the construction site, the amounts of packaging
materials included in the LCA calculations must be declared as Declared product properties (at Corresponds to the
technical scenario information for Module A5. the gate) and finishes specifications of EN -
1307
An assumed quality of work,
Conforms to the
when installed in accordance
Transport to the construction site (A4) manufacturer's -
with the manufacturer’s
Name Value Unit instructions
instructions
Litres of fuel (truck, EURO 0-6 mix) 0.0102 l/100km
Usage conditions, e.g. Use in areas defined by
Transport distance 700 km frequency of use, mechanical the use class according -
Capacity utilisation (including empty runs) 55 % exposure to EN 1307
Maintenance e.g. required According to the
Installation in the building (A5)
frequency, type and quality and manufacturers -
Name Value Unit replacement of components instructions
Material loss 0.131 kg
End of Life (C1-C4)
Polyethylene packaging waste and installation waste are
Three different end-of-life scenarios are declared and the
considered to be
results are indicated separately in module C.
incinerated in a municipal waste incineration plant. Cardboard
Each scenario is calculated as a 100% scenario.
packaging
Scenario 1: 100 % landfill disposal
waste is going to be recycled.
Scenario 2: 100 % municipal waste incineration (MWI)
Preparation of the floor and auxiliaries (adhesives, fixing
with R1 > 0.6
agents, PET connectors etc.) are not taken into account.
Scenario 3: 100 % recovery in the cement industry
Maintenance (B2) If combinations of these scenarios have to be calculated this
The values for cleaning refer to 1 m2 floor covering per year. should be done according to the following scheme:
Depending EOL-impact = x % impact (Scenario 1)
on the application based on ISO 10874, the technical service + y % impact (Scenario 2)
4 Environmental-Product Declaration - Interface - Continuously dyed tufted tiles, 100% rec PA 6, a CQuest Bio Sone backing
+ z % impact (Scenario 3) scenario information
with x % + y % + z % = 100 % Recovery or recycling potentials due to the three end-of-life
Name ValueUnit scenarios (module C) are indicated separately.
Collected as mixed construction waste (scenario 1
4.356 kg Recycling in the cement industry (scenario 3)
and 2)
The
Collected separately (scenario 3) 4.356 kg
organic material of the carpet is used as an alternative fuel in a
Landfilling (scenario 1) 4.356 kg cement
Energy recovery (scenario 2) 4.356 kg kiln. It mainly substitutes for lignite (68.8%), hard coal (23.6%)
Energy recovery (scenario 3) 2.314 kg and
petrol coke (7.6%). The inorganic material is substantially
Recycling (scenario 3) 2.042 kg
integrated into the cement clinker and substitutes for original
material input. VDZ e.V.
Reuse, recovery and/or recycling potentials (D), relevant
5 Environmental-Product Declaration - Interface - Continuously dyed tufted tiles, 100% rec PA 6, a CQuest Bio Sone backing
LCA: Results
The LCA results refer to all declared products with a maximum total pile weight of 1215 g/m2. LCA results for
products with a maximum total pile weight of 580 g/m2 can be taken from the corresponding tables of the annexe.
Results for specific products with any other total pile weight can be calculated by using equation 1 given in the
annexe (see annexe chapter: 'General Information on the annexe'). The declared result figures in module B2 have
to be multiplied by the assumed service life (in years) of the floor covering in the building under consideration.
Information on non-relevant modules: Modules B3 - B7 are not relevant during the service life of the carpet.
Modules C1, C3/1, C4/2 and C4/3 cause no additional impact (see chapter "LCA: Calculation rules" in this
document). All these modules are declared and marked as 'modules not relevant/declared'. Module C2 represents
the transport for scenarios 1, 2 and 3. Column D represents benefits from module A5 assembly.
DESCRIPTION OF THE SYSTEM BOUNDARY (X = INCLUDED IN LCA; ND = MODULE OR INDICATOR NOT DECLARED; MNR =
MODULE NOT RELEVANT)
BENEFITS
AND LOADS
CONSTRUCTION
BEYOND
PRODUCT STAGE PROCESS USE STAGE END OF LIFE STAGE
THE SYSTEM
STAGE
BOUNDARIE
S
la ire ta m w a Ry lp p u s tro p s n a rT g n iru tc a fu n a M e h t m o rf tro p s n a rTe tis e h t o t e ta g y lb m e s s A e s U e c n a n e tn ia M ria p e R tn e m e c a lp e R tn e m h s ib ru fe R y g re n e la n o ita re p Oe s u re ta w la n o ita re p Oe s u n o itc u rts n o c -e Dn o itilo m e d tro p s n a rT g n is s e c o rp e ts a W la s o p s iD -e s u e R-y re v o c e R-g n ilc y c e Rla itn e to p
A1 A2 A3 A4 A5 B1 B2 B3 B4 B5 B6 B7 C1 C2 C3 C4 D
X X X X X X X MNR MNR MNR MND MND X X X X X
RESULTS OF THE LCA - ENVIRONMENTAL IMPACT according to EN 15804+A2: 1 m² floor covering
Parameter Unit A1-A3 A4 A5 B1 B2 C1 C2 C3/2 C3/3 C4/1 D D/1 D/2 D/3
kg
GWP-total 3.97E+00 2.67E-01 3.81E-01 0 4.16E-01 0 1.48E-02 5.65E+00 5.7E+00 1.25E+00 -2.12E-02 0 -2.53E-01 -1.63E-01
CO -Äq.
2
kg
GWP-fossil 5.23E+00 2.62E-01 3.64E-01 0 2.15E-01 0 1.45E-02 4.7E+00 4.75E+00 3.05E-01 -2.11E-02 0 -2.52E-01 -1.63E-01
CO -Äq.
2
GWP- kg -1.27E
3.39E-03 1.74E-02 0 4.16E-03 0 1.88E-04 9.49E-01 9.49E-01 9.48E-01 -1.08E-04 0 -1.27E-03 -2.78E-04
biogenic CO 2-Äq. +00
kg
GWP-luluc 9.55E-03 1.48E-03 3.41E-04 0 1.96E-01 0 8.22E-05 2.13E-04 4.23E-04 1.5E-04 -2.31E-06 0 -2.71E-05 -7.89E-05
CO -Äq.
2
kg CFC11-
ODP 2.54E-08 1.59E-14 7.62E-10 0 3.42E-08 0 8.83E-16 4.76E-13 8.05E-13 4.15E-13 -1.42E-13 0 -1.66E-12 -2.06E-13
Äq.
AP mol H+-Äq. 2.14E-02 1.58E-03 8.73E-04 0 8.32E-04 0 8.78E-05 5.89E-03 6.16E-03 9.15E-04 -2.77E-05 0 -3.26E-04 -6.26E-04
EP- kg
1.5E-04 7.93E-07 4.53E-06 0 5.19E-06 0 4.4E-08 7.79E-07 9.55E-07 5.76E-05 -2.89E-08 0 -3.38E-07 -1.76E-07
freshwater PO 4-Äq.
EP-marine kg N-Äq. 7.21E-03 7.77E-04 3.29E-04 0 1.97E-04 0 4.31E-05 2.91E-03 3.03E-03 2.02E-04 -7.53E-06 0 -8.9E-05 -1.88E-04
EP-terrestrial mol N-Äq. 6.55E-02 8.6E-03 3.23E-03 0 2.83E-03 0 4.77E-04 3.24E-02 3.37E-02 2.22E-03 -8.07E-05 0 -9.54E-04 -2.06E-03
kg
POCP NMVOC- 1.76E-02 1.47E-03 8.01E-04 4.18E-04 9.83E-04 0 8.15E-05 7.46E-03 7.69E-03 6.51E-04 -2.11E-05 0 -2.5E-04 -5.61E-04
Äq.
ADPE kg Sb-Äq. 2.67E-06 2.22E-08 8.17E-08 0 2.3E-07 0 1.23E-09 2.64E-08 3.56E-08 2.14E-08 -3.18E-09 0 -3.73E-08 -1.57E-08
-4.27E -1.86E
ADPF MJ 8.17E+013.55E+002.66E+00 0 5.9E+00 0 1.97E-01 3.19E+004.08E+00 4.38E+00 -3.59E-01 0
+00 +01
m3 world-
WDP Äq. 1.88E+01 2.38E-03 5.9E-01 0 9.99E-02 0 1.32E-04 7.28E-01 7.34E-01 -3.28E-03 -2.22E-03 0 -2.59E-02 -2.35E-02
deprived
GWP = Global warming potential; ODP = Depletion potential of the stratospheric ozone layer; AP = Acidification potential of land and water; EP =
Eutrophication potential; POCP = Formation potential of tropospheric ozone photochemical oxidants; ADPE = Abiotic depletion potential for non-fossil
resources; ADPF = Abiotic depletion potential for fossil resources; WDP = Water (user) deprivation potential)
RESULTS OF THE LCA - INDICATORS TO DESCRIBE RESOURCE USE according to EN 15804+A2: 1 m² floor covering
Parameter Unit A1-A3 A4 A5 B1 B2 C1 C2 C3/2 C3/3 C4/1 D D/1 D/2 D/3
-1.15E
PERE MJ 7.51E+01 2.02E-01 2.95E+00 0 3.69E+00 0 1.12E-02 1.4E+01 1.42E+01 3.6E-01 -9.82E-02 0 -2.34E-01
+00
-1.34E -1.34E
PERM MJ 1.37E+01 0 -2.6E-01 0 0 0 0 0 0 0 0 0
+01 +01
-1.15E
PERT MJ 8.88E+01 2.02E-01 2.69E+00 0 3.69E+00 0 1.12E-02 5.19E-01 7.72E-01 3.6E-01 -9.82E-02 0 -2.34E-01
+00
-4.27E
PENRE MJ 7.45E+013.56E+00 3.06E+00 0 5.9E+00 0 1.98E-01 1E+01 1.09E+01 4.38E+00 -3.59E-01 0 -1.86E+01
+00
-6.86E -6.86E
PENRM MJ 7.25E+00 0 -3.96E-01 0 0 0 0 0 0 0 0 0
+00 +00
PENRT MJ 8.18E+013.56E+00 2.67E+00 0 5.9E+00 0 1.98E-01 3.19E+00 4.09E+00 4.38E+00 -3.59E-01 0 -4.27E -1.86E+01
6 Environmental-Product Declaration - Interface - Continuously dyed tufted tiles, 100% rec PA 6, a CQuest Bio Sone backing
+00
SM kg 3.71E+00 0 1.11E-01 0 0 0 0 0 0 0 0 0 0 1.3E-01
RSF MJ 0 0 0 0 0 0 0 0 0 0 0 0 0 0
NRSF MJ 0 0 0 0 0 0 0 0 0 0 0 0 0 0
FW m3 4.5E-01 2.28E-04 1.41E-02 0 3.34E-03 0 1.27E-05 1.72E-02 1.75E-02 5.13E-05 -9.39E-05 0 -1.1E-03 -1.75E-03
PERE = Use of renewable primary energy excluding renewable primary energy resources used as raw materials; PERM = Use of renewable primary
energy resources used as raw materials; PERT = Total use of renewable primary energy resources; PENRE = Use of non-renewable primary energy
excluding non-renewable primary energy resources used as raw materials; PENRM = Use of non-renewable primary energy resources used as raw
materials; PENRT = Total use of non-renewable primary energy resources; SM = Use of secondary material; RSF = Use of renewable secondary fuels;
NRSF = Use of non-renewable secondary fuels; FW = Use of net fresh water
RESULTS OF THE LCA – WASTE CATEGORIES AND OUTPUT FLOWS according to EN 15804+A2:
1 m² floor covering
Parameter Unit A1-A3 A4 A5 B1 B2 C1 C2 C3/2 C3/3 C4/1 D D/1 D/2 D/3
HWD kg 3.42E-03 1.7E-11 1.03E-04 0 4.19E-05 0 9.46E-13 4.88E-10 5.25E-10 6.76E-10 -4.87E-11 0 -5.83E-10 -1.36E-10
NHWD kg 6.03E-01 5.1E-04 4.93E-02 0 7.3E-03 0 2.83E-05 1.03E+00 1.03E+00 4.34E+00 -1.81E-04 0 -2.13E-03 -7.94E-02
RWD kg 2.87E-03 4.38E-06 8.98E-05 0 3.76E-04 0 2.43E-07 1.13E-04 1.78E-04 5.38E-05 -2.82E-05 0 -3.29E-04 -5.15E-05
CRU kg 0 0 0 0 0 0 0 0 0 0 0 0 0 0
MFR kg 0 0 1.21E-01 0 0 0 0 0 1.17E+00 0 0 0 0 0
MER kg 0 0 0 0 0 0 0 0 0 0 0 0 0 0
EEE MJ 0 0 2.91E-01 0 0 0 0 7.65E+00 0 0 0 0 0 0
EET MJ 0 0 5.34E-01 0 0 0 0 1.41E+01 6.92E+01 0 0 0 0 0
HWD = Hazardous waste disposed; NHWD = Non-hazardous waste disposed; RWD = Radioactive waste disposed; CRU = Components for re-use;
MFR = Materials for recycling; MER = Materials for energy recovery; EEE = Exported electrical energy; EET = Exported thermal energy
RESULTS OF THE LCA – additional impact categories according to EN 15804+A2-optional:
1 m² floor covering
Parameter Unit A1-A3 A4 A5 B1 B2 C1 C2 C3/2 C3/3 C4/1 D D/1 D/2 D/3
Disease
PM 1.63E-07 9.14E-09 5.92E-09 0 6.84E-08 0 5.07E-10 2.4E-08 2.57E-08 8.79E-09 -2.3E-10 0 0 -8.73E-09
incidence
kBq U235-
IR 4.66E-01 6.42E-04 1.45E-02 0 6.78E-02 0 3.56E-05 1.71E-02 2.82E-02 7.95E-03 -4.77E-03 0 0 -6.16E-03
Äq.
ETP-fw CTUe 8.3E+01 2.47E+00 2.62E+00 3.6E-03 2.69E+00 0 1.37E-01 1.51E+00 2.03E+00 4.29E+00 -7.85E-02 0 0 -3.38E+00
HTP-c CTUh 2.66E-09 4.98E-11 8.39E-11 0 6.21E-10 0 2.76E-12 7.51E-11 8.72E-11 1.93E-10 -3.62E-12 0 0 -4.42E-11
HTP-nc CTUh 7.67E-08 2.96E-09 2.55E-09 2.6E-11 9.46E-09 0 1.64E-10 4.94E-09 5.54E-09 1.61E-08 -1.39E-10 0 0 -2.75E-09
SQP SQP ND ND ND ND ND 0 6.11E-02 6.49E-01 9.33E-01 2.84E-01 ND ND ND ND
PM = Potential incidence of disease due to PM emissions; IR = Potential Human exposure efficiency relative to U235; ETP-fw = Potential comparative
Toxic Unit for ecosystems; HTP-c = Potential comparative Toxic Unit for humans (cancerogenic); HTP-nc = Potential comparative Toxic Unit for humans
(not cancerogenic); SQP = Potential soil quality index
No substantiated values can be given for the SQP indicator with the existing database.
The result
figures given in module B2 refer to a period of 1 year because a reference service life is not declared. They have to be
multiplied by the assumed service life (in years) of the floor covering
in the building under consideration.
Disclaimer 1 – for the indicator “Potential Human exposure efficiency relative to U235”.
This impact category deals mainly with the eventual impact of low dose ionizingradiation on human health of the nuclear fuel cycle. It
does not consider effects due to possible nuclear accidents, occupational exposure nor due to radioactive waste disposal in
undergroundfacilities. Potential ionizing radiation from the soil, from radon and from some construction materials is also not measured
by this indicator.
Disclaimer 2 – for the indicators “abiotic depletion potential for non-fossil resources”, “abiotic depletion potential for fossil resources”,
“water (user) deprivation potential, deprivation-weighted water consumption”, “potential comparative toxic unit for ecosystems”,
“potential comparative toxic unit for humans – cancerogenic”, “Potential comparative toxic unit for humans - not cancerogenic”,
“potential soil quality index”.
The results of this environmental impact indicator shall be used with care as the uncertainties on these results are high or as there is
limited experienced with the indicator.
References
EN 1307 building elements - Part 1: Classification using data from
DIN EN 1307: 2014+A1:2016+A2:2018-05: Textile floor reaction to
coverings - Classification fire tests
EN 14041
EN 13501-1 DIN EN 14041: 2018-05 and DIN EN 14041: 2008-05:
DIN Resilient, textile and laminate floor coverings - Essential
EN 13501-1:2019-05: Fire classification of construction characteristics
products and EN 15804
7 Environmental-Product Declaration - Interface - Continuously dyed tufted tiles, 100% rec PA 6, a CQuest Bio Sone backing
DIN EN
15804:2012+A2:2019 + AC:2021, Sustainability of construction
works —
Environmental Product Declarations — Core rules for the
product category
of construction products
EN 16810
DIN ecoinvent
EN 16810: 2017-08: Resilient, textile and laminate floor ecoinvent, Zurich, Switzerland, database version 3.7, published
coverings – September 2020
Environmental product declarations – Product category rules
ISO 10874
DIN EN ISO 10874: 2012+A1:2021-04: Resilient, textile and
laminate floor coverings - Classification GaBi database
ISO 14025
DIN GaBi Software-System and Database for Life Cycle
EN /ISO 14025:2011-10/, Environmental labels and Engineering, version
declarations — Type 10.5 Sphera, Leinfelden-Echterdingen, database version 2022-
III environmental declarations — Principles and procedures 1
ISO 14040 PCR Part A
DIN EN ISO 14040:2006+A1:2020 Environmental
management - Life cycle assessment - Principles and Product
framework Category Rules for Building-Related Products and Services
Part A: Calculation Rules for the
ISO 14044 Life Cycle Assessment and Requirements on the Project Report
DIN EN ISO 14044:2006+A1:2018+A2:2020 Environmental according to EN 15804+A2:2019, V1.2,
management - Life cycle assessment - Requirements and Berlin: Institut Bauen und Umwelt e.V. (IBU), November 2021
guidelines
ISO 15686
ISO 15686: Buildings and constructed assets -
Service life planning
ISO 15686-1: 2011-05: Part 1: General principles and PCR Part B
framework
ISO 15686-2: 2012-05: Part 2: Service life prediction Product
procedures Category Rules for Building-Related Products and Services
ISO 15686-7: 2017-04: Part 7: Performance Part B: Requirements on the EPD for floor coverings, V1.2,
evaluation for feedback of service life data Berlin: Institut Bauen und Umwelt e.V. (IBU), February 2018
from practice
ISO 15686-8: 2008-06: Part 8: Reference service life
and service-life estimation
Regulation (EU) No. 305/2011 PRODIS
Regulation
No. 305/2011 Construction Products Regulation (CPR) of the Product
European Information System (PRODIS) of the European Carpet Industry,
Council and of the European Parliament, April 2011 Gemeinschaft umweltfreundlicher Teppichboden e.V (GUT) and
European
General Instructions for the IBU-EPD Program Carpet and Rug Association
General Instructions for the EPD-Program of the Institut Bauen
und Umwelt e.V., The Preparation of Environmental Product (ECRA), http://www.pro-dis.info
Declarations - EPDs, version 2.0, Institut Bauen und Umwelt
e.V., Berlin, January 2021, www.ibu-epd.de
REACH
BNB, Nutzungsdauer von Bauteilen
Bewertungssystem Regulation
Nachhaltiges Bauen (BNB), Nutzungsdauer von Bauteilen, (EC) No 1907/2006 of the European Parliament and of the
Bundesministerium des Inneren, für Bau und Heimat, Council of 18
24.02.2017 December 2006 concerning the Registration, Evaluation,
Authorisation and
Restriction of Chemicals (REACH), June 2017, last update:
08.07.2021
ECHA candidate list
Candidate
List of substances of very high concern (SVHCs) for
authorisation, VDZ e.V.
08.07.2021, European Chemicals Agency (ECHA), Helsinki,
Finland Association of German Cement Works, Ed. Environ-mental
8 Environmental-Product Declaration - Interface - Continuously dyed tufted tiles, 100% rec PA 6, a CQuest Bio Sone backing
Data of the German Cement Industry 2020 in the EPD do not need to be listed here again.
The literature referred to in the Environmental Product The current version of PCR Part A and PCR Part B of the PCR
Declaration must be listed in full.Standards already fully quoted document on which they are based must be referenced.
9 Environmental-Product Declaration - Interface - Continuously dyed tufted tiles, 100% rec PA 6, a CQuest Bio Sone backing
Publisher
Institut Bauen und Umwelt e.V. +49 (0)30 3087748- 0
Hegelplatz 1 info@ibu-epd.com
10117 Berlin www.ibu-epd.com
Germany
Programme holder
Institut Bauen und Umwelt e.V. +49 (0)30 3087748- 0
Hegelplatz 1 info@ibu-epd.com
10117 Berlin www.ibu-epd.com
Germany
Author of the Life Cycle Assessment
Gemeinschaft umweltfreundlicher Teppichboden +49 (0)241 96843 410
(GUT) e.V. mail@gut-ev.de
Schönebergstraße 2 www.gut-ev.org
52068 Aachen
Germany
Owner of the Declaration
Interface Europe Manufacturing BV +31 33 277 55 55
Industrielaan 15 receptie@interface.com
3925ZG Scherpenzeel www.interface.com
Netherlands
10 Environmental-Product Declaration - Interface - Continuously dyed tufted tiles, 100% rec PA 6, a CQuest Bio Sone backing
