ENVIRONMENTAL PRODUCT DECLARATION
as per ISO 14025 and EN 15804+A2
Owner of the Declaration Armacell International S.A.
Programme holder Institut Bauen und Umwelt e.V. (IBU)
Publisher Institut Bauen und Umwelt e.V. (IBU)
Declaration number EPD-ARM-20220038-IBB1-EN
Issue date 22.03.2022
Valid to 21.03.2027
AF/ArmaFlex Evo insulation for building equipment and
industrial installation
Armacell GmbH
www.ibu-epd.com | https://epd-online.com
Umwelt Produktdeklaration Name des Herstellers – Name des Produkts
1. General Information
Armacell GmbH AF/ArmaFlex Evo
Programme holder Owner of the declaration
IBU – Institut Bauen und Umwelt e.V. Armacell International S.A.
Panoramastr. 1 Robert-Bosch-Str. 10
10178 Berlin 48153 Münster - Germany
Germany
Declaration number Declared product / declared unit
EPD-ARM-20220038-IBB1-EN 1m³ insulation material AF/ArmaFlex Evo
This declaration is based on the product Scope:
category rules: Product line AF/ArmaFlex Evo
Insulating materials made of foam plastics, 01.2019 Insulation material for industrial and building
(PCR checked and approved by the SVR) installations vulcanized in tubes and sheets.
This declaration is an Environmental Product
Issue date Declaration according to ISO 14025 describing the
22.03.2022 average environmental performance of the product
produced in Germany, Spain and Poland. The average
Valid to has been calculated based on site specific annual
production volumes.
21.03.2027
As the installation of the product is not restricted to
countries where the products have been produced the
validity of this EPD is considered at least EU wide.
The owner of the declaration shall be liable for the
underlying information and evidence; the IBU shall not
be liable with respect to manufacturer information, life
cycle assessment data and evidences.
The EPD was created according to the specifications
of EN 15804+A2. In the following, the standard will be
simplified as EN 15804.
Verification
The standard EN 15804 serves as the core PCR
Independent verification of the declaration and data
according to ISO 14025:2011
Dipl. Ing. Hans Peters internally x externally
(chairman of Institut Bauen und Umwelt e.V.)
Dr. Alexander Röder Vito D'Incognito
(Managing Director Institut Bauen und Umwelt e.V.)) (Independent verifier)
2. Product
2.1 Product description/Product definition (FEF) products – Specification and the CE-marking.
AF/ArmaFlex Evo is the professional, highly-flexible, For the application and use the respective national
closed-cell elastomeric foam insulation (FEF) for provisions apply.
continuous energy saving and condensation control 2.2 Application
purposes. The combination of very low thermal AF/ArmaFlex Evo is used to insulate pipes, air ducts
conductivity and extremely high resistance to water and vessels including fittings and flanges of industrial
vapour transmission prevents long-term energy losses installations and building equipment.
and water vapour ingress and reduces the risk of  Condensation control, energy saving and
corrosion under insulation. noise control in refrigeration and air
conditioning equipment and process plants.
For the placing on the market of the product in the
 Energy saving according to local energy-
European Union/European Free Trade Association
(EU/EFTA) (with the exception of Switzerland) saving laws, prevention of heat loss and noise
Regulation (EU) No. 305/2011 (CPR) applies. The reduction of heating and plumbing systems.
product needs a declaration of performance taking into  Condensation control and noise reduction in
consideration EN 14304:2013-04 , Thermal insulation service-water and waste-water systems.
products for building equipment and industrial
installations – Factory made flexible elastomeric foam
2 Environmental Product Declaration Armacell GmbH – AF/ArmaFlex Evo insulation for industrial and building installation
 Condensation control, energy saving and
noise control in refrigeration and air- This product/article/at least one partial article contains
other CMR substances in categories 1A or 1B which
conditioning equipment in the ship-building
are not on the candidate list, exceeding 0.1 percentage
sector.
by mass: No
Biocide products were added to this construction
2.3 Technical Data product or it has been treated with biocide products
(this then concerns a treated product as defined by the
(EU) Ordinance on Biocide Products No. 528/2012):
Constructional data
Name Value Unit Yes, AF/ArmaFlex Evo is treated with the antimicrobial
Gross density 52.5 kg/m3 biocide pyrithione zinc.
Water vapour diffusion resistance ≥ 10000/
-
factor acc. to EN 12086, EN 13469/ ≥ 7000 The products may contain traces of azodicarbonamide
0,033/0, (ADCA). Possible minimal residual amounts are
Thermal conductivity 036 W/(mK) included in the polymer matrix. A health impairment
(0°C) can be excluded. For the production of insulation
Maximum service temperature acc. to material based on synthetic rubber, there is presently
+110 °C
EN 14706, EN 14707 no alternative to ADCA available.
Minimum service temperature -50 °C
Tubes: Synthetic rubber determines the flexibility;
BL-s2, Fillers determine the fire properties and firmness;
Reaction to fire acc. to EN 13501-1 d0/ - Blowing agent causes the expansion process during
Sheets: manufacturing;
B-s2, d0 Accelerator and sulphur enable the vulcanisation;
Structure-borne sound transmission Plasticizers determine the flexibility;
acc. to EN ISO 3822-1 ≤ 28 dB(A) Flame retardants ensure fire resistance.
Weighted sound absorption coefficient
≤ 0,45 -
αw acc. to EN ISO 11654
2.6 Manufacture
ArmaFlex Evo products are manufactured in a
Insulation materials on the basis of synthetic rubber do
pressureless, continuous and discontinuous production
not absorb moisture from the air. For this reason the
process.
normal building moisture does not lead to an increase
In the first step, a homogenous compound is produced
in thermal conductivity.
with rubber, additives, ancillary materials, blowing and
vulcanization agents. This is done on the rolling mill or
Performance data of the product in accordance with
in the internal mixer followed by the rolling mill.
the declaration of performance with respect to its
Rubber extruders are used to process the compounds
essential characteristics according to EN 14304:2013-
to produce raw profiles with defined dimensions. Here
04, Thermal insulation products for building equipment
exact compliance with the dimensions for the raw
and industrial installations – Factory made flexible
profile is crucial for the dimensional accuracy of the
elastomeric foam (FEF) products – Specification
foamed product.
In the case of the discontinuous, pressureless
2.4 Delivery status
production process, the raw profiles are cut to length
FEF made of cross-linked elastomer is supplied as
and then foamed in a hot-air oven. In the case of the
sheets, tubes and shaped pieces. Products with self-
continuous, pressureless process, the extruded profile
adhesive backings/closures are available; these
is fed directly onto a vulcanization line whose energy
variations are not included in the calculations.
source may be hot air.
Insulation thicknesses are available for all common
In foam production, vulcanization and blowing
pipe diameters up to an outer diameter of 168 mm
processes run alongside each other. Both reactions
(tubes).
are regulated by temperature control. Recipe and
temperature control determine the properties of the
2.5 Base materials/Ancillary materials
foam.
Quality assurance:
ArmaFlex Evo is a highly flexible insulation material
EC Certificate of conformity no. 0543 of the
based on synthetic rubber, which consists of around 20
Gütegemeinschaft Hartschaum e.V. Celle.
basic components. The following table displays the
Quality management system in accordance with EN
composition split into functional substance groups.
ISO 9001.
Name Value Unit
Rubber and polymers 19 %
2.7 Environment and health during
Fillers and pigments 7 %
manufacturing
Blowing agent 12 %
During all manufacturing steps and at all production
Vulcanisation system, additives,
24 % sites of Armacell, the production follows the national
plasticisers
guidelines and regulations. A regenerative thermal
Flame retardant 38 %
oxidizer is installed to treat exhaust air.
Certification of the environmental management system
This product/article/at least one partial article contains
is in accordance with ISO 14001.
substances listed in the candidate list (date:
17.01.2022) exceeding 0.1 percentage by mass: No
3 Environmental Product Declaration Armacell GmbH – AF/ArmaFlex Evo insulation for industrial and building installation
2.8 Product processing/Installation
The product is installed by using knives. No special 2.13 Extraordinary effects
tools, nor specific protection is necessary.
When applying adhesives the information given in the Fire
relevant safety data sheets is to be heeded. According to /EN 13501/, ArmaFlex Evo is classified as
The recommendations for installing the product a combustible insulation material. Due to its material
depend on the product and system and are described structure it does not contribute to an uncontrollable
in the respective documents (e.g. application manuals) spread of fire under installation conditions typical on a
or the data sheets. More details under building site. ArmaFlex Evo does not drip under
www.armacell.com. practical fire conditions, this means that fire spread is
ruled out. The product is self-extinguishing and
therefore only makes a minor contribution to the actual
2.9 Packaging fire event. There is no possibility of the material self-
As a rule, ArmaFlex Evo products are packaged in igniting. ArmaFlex Evo does not propagate the fire
cardboard boxes and transported on reusable pallets either horizontally or vertically.
(For the LCA calculation of this EPD though, 100%
incineration is assumed). Over-sized rolls of sheet Fire protection
material are packaged in polyethylene (PE) foil. The Name Value
cardboard boxes are usually recycled through Euro class Tubes: BL / Sheets B
Interseroh’s dual system. Burning droplets Tubes/Sheets: d0
Smoke development Tubes/Sheets: s2
2.10 Condition of use Water
When the products are used for the purpose for which Armacell insulation materials have a high resistance to
they are intended, there are no changes in the material water vapour transmission which keeps possible water
composition during use, except in the event of vapour transmission processes to a minimum
extraordinary impacts (see 2.14). permanently. Therefore, a significant reduction in the
insulation effect can be ruled out permanently.
2.11 Environment and health during use If the insulation material is exposed to water over a
Ingredients: There are no particular aspects of the long period of time (e.g. flooding) it should be replaced.
material composition during use.
Eurofins Product Testing A/S has tested a wide range Mechanical destruction
and varieties of typical FEF (Flexible Elastomeric ArmaFlex Evo insulation materials are flexible foams
Foam) products marketed in the EU from CEFEP and thus display limited mechanical stability.
(European Group of FEF manufacturers). Sampling, Therefore, if the material will be subject to greater
testing and evaluation were performed according to mechanical impact it should be protected
CEN TS 16516, AgBB, ISO 16000-3, ISO 16000-6, appropriately, e.g. by a metal jacket or Arma-Chek
ISO 16000-9, ISO 16000-11 in the latest versions. covering.
Based on the loading factor 0.05 m²/m³, which was ArmaFlex Evo products are not UV resistant. If the
determined after consideration of real life applications material is subject to UV-rays it should be protected
with FEF products (in living rooms) and accordingly.
recommendation of experts of the test institute, all
results were clearly below the limit values. For 2.14 Re-use phase
example, the determined total volatile organic If removed properly the product can be re-used.
compound (TVOC) after 28 days was for all samples Correctly sorted material can be ground and used to
below 100 mg/m3. Certificates are available on manufacture new products (e.g. ArmaSound). For the
request. LCA calculation of this EPD though, 100% incineration
is assumed.
2.12 Reference service life 2.15 Disposal
ArmaFlex Evo products are long-lasting products. Dispose of the materials according to local regulations.
Findings show that when used and installed properly Regulated by the European Waste Catalogue: Waste
they can have an estimated service life of more than code 07 02 13 (waste plastic).
50 years. It is practically only restricted by the service Note: Please observe Commission Decision
life of the equipment or whole building, which can 2001/118/EC.
extent that time period. The insulation performance is
almost completely maintained over the entire service 2.16 Further information
life. The insulation performance is only compromised Further information on ArmaFlex® can be found on the
by extraordinary impacts and damage during manufacturer’s website www.armacell.com. Detailed
construction specification clauses for the products are provided at
www.armaflex.de.
3. LCA: Calculation rules
3.1 Declared Unit As additional information and support for installers the
The declaration refers to 1 m³ insulation product. thermal conductivity coefficient (lambda-value) and R-
For the LCA calculations the average density per value per 20 cm thickness per product brand are given.
product brand is used.
Declared unit
4 Environmental Product Declaration Armacell GmbH – AF/ArmaFlex Evo insulation for industrial and building installation
Name Value Unit Approximations are used with the consideration of
Declared unit 1 m3 similar supply chain effort or similar elementary
Gross density 52.5 kg/m3 composition. Partly an estimation is modelled using
pre-products of the specific material and adding an
Thermal conductivity λ : 0.033 W/(mK (0°C) energy effort as well as considering the treatment of
R-value – thickness: 20 cm: 6.1 (m²K)/W production residues for this step in the supply chain.
3.4 Cut-off criteria
In the assessment, all reported data from the
3.2 System boundary production process are considered, utilised thermal
The data collection refers to the yearly production in energy, and electric power consumption using best
2020. The following life cycle stages are considered: available life cycle inventory (LCI) datasets. Thus
material and energy flows contributing less than 1% of
Type of EPD: Cradle-to-Gate with options. mass or energy are considered.
No cut-off criteria are applied in the foreground data in
Production A1-A3: this study.
The LCA calculation covers the production of the raw For cut-off criteria in the background system, see
materials (supply chain – A1), the mixing of raw information provided in the modelling principles and
materials according to the respective recipes specific documentations (documentation.gabi-
(MasterBatch) exclusively done in Münster, Germany, software.com).
the transport (A2) of the MasterBatches to the
production facility for foaming and the foaming process 3.5 Background data
(A3) in Germany, Spain or Poland, including the The LCA model is created using the GaBi ts Software
packaging material. system (v10) for life cycle engineering, developed by
Transport A4: Sphera. The GaBi LCI database provides the life cycle
Average values for the transport from factory gate to inventory data for several of the raw and process
construction site are assumed. materials obtained from the background system. The
Installation A5: most recent update of the database was 2021 (Service
The installation considers the production of off-cuts, Pack CUP 2021.02)
incineration of these off-cuts and the disposal scenario
for the packaging material. Auxiliaries like adhesives or 3.6 Data quality
tapes or energy for installation are not considered. The foreground data collected by the manufacturer are
End-of-life C2, C3: based on yearly production amounts and
An incineration scenario for the used and demolished extrapolations of measurements on specific machines
product, including an assumption for the transport to and plants.
disposal, is covered. As the average environmental performance of the
Benefits for the next product system D: product brand has been calculated by a weighting of
Credits for electrical and thermal energy resulting from the site-specific production volumes the results also
the waste incineration process of the off-cut material show a representative picture regarding site specific
and packaging (A5) and the product (C3) are declared production technologies. The average results therefore
in module D. can be assessed as robust.
Most of the necessary life cycle inventories for the
basic materials are available in the GaBi database.
3.3 Estimates and assumptions The last update of the database was in 2021 (Service
Scenario assumptions: Pack CUP 2021.02)
Installation (A5): Further LCIs for materials of the supply chain of the
The additional demand of material for installation basic materials are approximated with LCIs of similar
depends on the specific frame conditions of the materials or estimated by the combination of available
building and pipe system to be insulated. Parts of the LCIs.
product can be joined; thus installation off-cut is very For electrical and thermal energy regional specific grid
small. A loss of 1% is assumed. mixes and regional specific supply for natural gas are
Transport to customer (A4): considered.
Armacell’s data collectors reported average figures for
the distribution of their material. Depending on the 3.7 Period under review
country, the transport distance varies from 500 km to The production data refer to an average of the year
800 km 2020.
End-of-life (C2, C3):
The transport from place of usage to a waste 3.8 Allocation
incineration plant is assumed as 100 km. Allocation of upstream data:
After the demolition of the product a current realistic For all refinery products, allocation by mass and net
End-of-life scenario is the incineration of the material. calorific value is applied. The specific manufacturing
According to the reported net calorific value of the route of every refinery product is modelled and so the
materials and the elementary composition, a partial impacts associated with the production of these
stream consideration for the incineration process of products are calculated individually.
PVC-products is applied as an approximation for all Materials and chemicals used in the manufacturing
declared products. process are modelled using the allocation rule most
Inventory estimations and approximations: suitable for the respective product. For further
The reported recipes for the rubber mixes contain information on a specific product see
specific substances of the rubber industry. For these documentation.gabi-software.com.
materials only partly life cycle inventories are available. Allocation in the foreground data:
5 Environmental Product Declaration Armacell GmbH – AF/ArmaFlex Evo insulation for industrial and building installation
Part of the production residues (ca. 2%) are used for The credits for thermal and electrical energy are
the manufacturing of a non-declared product calculated via inversion of the life cycle inventory of
(ArmaSound). These materials leave the process European average data.
without further consideration of any treatment and Allocation for waste paper:
without credit (cut-off-approach). Paper/corrugated board is used as packaging material
No further allocation is applied in the software model. and this usually includes a mix of recycled and virgin
The overall production of the Armacell production fibres. When modelling the production of paper, the
facilities comprises further products beside the scrap paper that is used in this process has been
products considered in this study. Data for thermal and assumed to be burden free. Similarly, waste paper
electrical energy, as well as auxiliary material, refer to arising in the product life cycle is assumed to be
the declared products only. During data collection the recycled. Robust data on paper and cardboard
allocation is done via mass, area, pieces or time spent recycling are not promptly available and refer to a very
in the machine, depending on the process step and complex system. Hence, to apply this methodology
reasonable split. The data collectors at Armacell consistently throughout the model, a cut-off approach
decided on the distribution basis. has been applied, i.e., input of waste paper is
Allocation for waste materials: considered without environmental burden, resulting
Production waste is sent to a waste incineration plant waste paper is not credited. The recycling process and
and to landfill (Spain). The resulting electrical and the production process of paper are merged in the
thermal energy from the incineration process is looped production process. The C-balance referring to fresh
inside module A1-A3. The quality of the recovered fibre is corrected via CO emissions (biotic)
2
energy is assumed to be the same as that of the input (assumption of final rotting or incineration in the time
energy. frame of 100 years).
Landfilling of plastic material is assumed not to deliver
any landfill gas. 3.9 Comparability
All applied incineration processes are displayed via a Basically, a comparison or an evaluation of EPD data
partial stream consideration for the combustion is only possible if all the data sets to be compared
process, according to the specific composition of the were created according to EN 15804 and the building
incinerated material. For the waste incineration plant context, respectively the product-specific
an R1-value of >0.6 is assumed. characteristics of performance, are taken into account.
Environmental burden of the incineration of installation
residues (off-cuts), packaging and the product in the The used background dataset DB has been GaBi
end-of-life scenario is assigned to the system (A5 or 2021 (Service Pack CUP 2021.02)
C3); resulting credits for thermal and electrical energy
are declared in module D.
4. LCA: Scenarios and additional technical information
Characteristic product properties
Information on biogenic Carbon The following technical information serves as a basis
for the declared modules. The values refer to the
The biogenic carbon content quantifies the amount of declared unit of 1 m³.
biogenic carbon in a construction product leaving the
factory gate, and it shall be separately declared for the Transport to the building site (A4)
product and for any accompanying packaging.If the Name Value Unit
total mass of biogenic carbon containing materials is 0.12 -
Litres of fuel l/100km
less than 5 % of the total mass of the product and 0.16
accompanying packaging, the declaration of biogenic 500 -
Transport distance km
carbon content may be omitted. The mass of 800
packaging containing biogenic carbon shall always be Capacity utilisation (including empty
85 %
declared. runs)
Note: 1 kg biogenic Carbon is equivalent to 44/12 kg of Installation into the building (A5)
CO2 Name Value Unit
Material loss 1 %
Estimated service life
Name Value Unit
Life Span according to the
50 a
manufacturer
Information on describing the biogenic Carbon
Content at factory gate End of life (C1-C4)
Name Value Unit Name Value Unit
Biogenic Carbon Content in Energy recovery in WIP 52,5 kg
0 kg C
product
Biogenic Carbon Content in Reuse, recovery and/or recycling potentials (D),
20.01 kg C
accompanying packaging relevant scenario information
The embodied biogenic carbon leaves the system in Module D includes the credits of the incineration
Module A5. processes from A5 (off-cut of product installation,
6 Environmental Product Declaration Armacell GmbH – AF/ArmaFlex Evo insulation for industrial and building installation
packaging waste) and C3 (incineration of the product).
A waste incineration plant with an R1-value > 0.6 is
assumed.
7 Environmental Product Declaration Armacell GmbH – AF/ArmaFlex Evo insulation for industrial and building installation
5. LCA: Results
The following information on environmental impacts is expressed with the impact category parameters of LCIA
using characterisation factors. The chosen characterisation factors fulfil the requirements of EN 15804.
Disclaimer:
EP-freshwater: This indicator has been calculated as “kg P eq” as required in the characterization model
(EUTREND model, Struijs et al., 2009b, as implemented in ReCiPe;
http://eplca.jrc.ec.europa.eu/LCDN/developerEF.xhtml)
DESCRIPTION OF THE SYSTEM BOUNDARY (X = INCLUDED IN LCA; ND = MODULE OR INDICATOR NOT
DECLARED; MNR = MODULE NOT RELEVANT)
BENEFITS AND
CONSTRUCTI LOADS
PRODUCT STAGE ON PROCESS USE STAGE END OF LIFE STAGE BEYOND THE
STAGE SYSTEM
BOUNDARIES
8 Environmental Product Declaration Armacell GmbH – AF/ArmaFlex Evo insulation for industrial and building installation
lairetam
waR
ylppus tropsnarT
gnirutcafunaM
eht
morf
tropsnarT
etis
eht
ot
etag
ylbmessA esU
ecnanetniaM
riapeR
tnemecalpeR tnemhsibrufeR
ygrene
lanoitarepO esu
retaw
lanoitarepO esu
noitcurtsnoc-eD
noitilomed tropsnarT
gnissecorp
etsaW
lasopsiD -esueR -yrevoceR -gnilcyceR laitnetop
A1 A2 A3 A4 A5 B1 B2 B3 B4 B5 B6 B7 C1 C2 C3 C4 D
X X X X X ND ND MNR MNR MNR ND ND ND X X ND X
RESULTS OF THE LCA - ENVIRONMENTAL IMPACT according to EN 15804+A2: 1 m³ AF/ArmaFlex Evo
insulation for industrial and building installation
Core Indicator Unit A1-A3 A4 A5 C2 C3 D
Global warming potential - total [kg CO2-Eq.] 1.40E+2 3.82E+0 8.05E+1 2.51E-1 1.36E+2 -3.76E+1
Global warming potential - fossil fuels [kg CO2-Eq.] 2.14E+2 3.79E+0 4.23E+0 2.49E-1 1.36E+2 -3.74E+1
Global warming potential - biogenic [kg CO2-Eq.] -7.51E+1 -4.84E-3 7.63E+1 -3.18E-4 2.75E-2 -1.87E-1
GWP from land use and land use change [kg CO2-Eq.] 2.98E-1 3.11E-2 3.78E-3 2.04E-3 3.05E-2 -2.58E-2
Depletion potential of the stratospheric ozone layer [kg CFC11-Eq.] 8.55E-10 4.85E-16 8.64E-12 3.19E-17 2.18E-13 -4.26E-13
Acidification potential, accumulated exceedance [mol H+-Eq.] 6.82E-1 1.11E-2 9.49E-3 7.27E-4 3.69E-2 -4.88E-2
Eutrophication, fraction of nutrients reaching freshwater
end compartment
[kg P4-Eq.] 2.60E-3 1.13E-5 2.70E-5 7.40E-7 3.36E-5 -4.87E-5
Eutrophication, fraction of nutrients reaching marine end
[kg N-Eq.] 1.59E-1 5.03E-3 2.48E-3 3.31E-4 1.23E-2 -1.39E-2
compartment
Eutrophication, accumulated exceedance [mol N-Eq.] 1.48E+0 5.63E-2 2.71E-2 3.70E-3 1.52E-1 -1.49E-1
Formation potential of tropospheric ozone photochemical
[kg NMVOC-Eq.] 6.23E-1 9.93E-3 8.64E-3 6.53E-4 3.58E-2 -3.90E-2
oxidants
Abiotic depletion potential for non-fossil resources [kg Sb-Eq.] 3.67E+3 5.05E+1 4.34E+1 3.32E+0 2.52E+2 -6.49E+2
Abiotic depletion potential for fossil resources [MJ] 4.71E-1 2.89E-7 4.76E-3 1.90E-8 3.11E-6 -6.21E-6
Water (user) deprivation potential, deprivation-weighted [m³ world-Eq
2.24E+1 3.29E-2 1.88E+0 2.17E-3 1.05E+1 -2.86E+0
water consumption (WDP) deprived]
RESULTS OF THE LCA - INDICATORS TO DESCRIBE RESOURCE USE according to EN 15804+A2: 1 m³
AF/ArmaFlex Evo insulation for industrial and building installation
Indicator Unit A1-A3 A4 A5 C2 C3 D
Renewable primary energy as energy carrier [MJ] 1.58E+3 2.82E+0 1.22E+2 1.85E-1 5.63E+1 -1.46E+2
Renewable primary energy resources as material utilization [MJ] 1.04E+2 0.00E+0 -1.04E+2 0.00E+0 0.00E+0 0.00E+0
Total use of renewable primary energy resources [MJ] 1.68E+3 2.82E+0 1.82E+1 1.85E-1 5.63E+1 -1.46E+2
Non-renewable primary energy as energy carrier [MJ] 2.76E+3 5.06E+1 5.10E+1 3.32E+0 1.15E+3 -6.49E+2
Non-renewable primary energy as material utilization [MJ] 9.06E+2 0.00E+0 -7.51E+0 0.00E+0 -8.98E+2 0.00E+0
Total use of non-renewable primary energy resources [MJ] 3.67E+3 5.06E+1 4.35E+1 3.32E+0 2.52E+2 -6.49E+2
Use of secondary material [kg] 3.14E+1 0.00E+0 3.14E-1 0.00E+0 0.00E+0 0.00E+0
Use of renewable secondary fuels [MJ] 0.00E+0 0.00E+0 0.00E+0 0.00E+0 0.00E+0 0.00E+0
Use of non-renewable secondary fuels [MJ] 0.00E+0 0.00E+0 0.00E+0 0.00E+0 0.00E+0 0.00E+0
Use of net fresh water [m³] 1.47E+0 3.23E-3 5.41E-2 2.12E-4 2.74E-1 -1.43E-1
RESULTS OF THE LCA – WASTE CATEGORIES AND OUTPUT FLOWS according to EN 15804+A2:
1 m³ AF/ArmaFlex Evo insulation for industrial and building installation
Indicator Unit A1-A3 A4 A5 C2 C3 D
Hazardous waste disposed [kg] 1.53E-5 2.55E-9 1.55E-7 1.68E-10 4.50E-8 -1.46E-7
Non-hazardous waste disposed [kg] 2.09E+1 7.51E-3 1.19E+0 4.94E-4 8.35E+1 -3.04E-1
Radioactive waste disposed [kg] 8.14E-2 6.12E-5 1.08E-3 4.02E-6 7.41E-3 -4.71E-2
Components for re-use [kg] 0.00E+0 0.00E+0 0.00E+0 0.00E+0 0.00E+0 0.00E+0
Materials for recycling [kg] 0.00E+0 0.00E+0 4.00E+1 0.00E+0 0.00E+0 0.00E+0
Materials for energy recovery [kg] 0.00E+0 0.00E+0 0.00E+0 0.00E+0 0.00E+0 0.00E+0
Exported electrical energy [MJ] 0.00E+0 0.00E+0 2.20E+1 0.00E+0 1.37E+2 0.00E+0
Exported thermal energy [MJ] 0.00E+0 0.00E+0 3.95E+1 0.00E+0 2.50E+2 0.00E+0
RESULTS OF THE LCA – additional impact categories according to EN 15804+A2-optional:
1 m³ AF/ArmaFlex Evo insulation for industrial and building installation
Indicator Unit A1-A3 A4 A5 C2 C3 D
Potential incidence of disease due to PM emissions [Disease
3.21E-5 6.16E-8 3.45E-7 4.05E-9 9.37E-7 -4.20E-7
Incidence]
Potential Human exposure efficiency relative to U235 [kBq U235-
8.33E+0 8.76E-3 1.21E-1 5.76E-4 7.71E-1 -7.72E+0
Eq.]
Potential comparative toxic unit for ecosystems [CTUe] 3.55E+3 3.65E+1 3.98E+1 2.40E+0 2.06E+2 -1.36E+2
Potential comparative toxic unit for humans - cancerogenic [CTUh] 6.77E-8 7.36E-10 8.72E-10 4.84E-11 8.29E-9 -6.18E-9
Potential comparative toxic unit for humans - not cancerogenic [CTUh] 5.73E-6 4.29E-8 7.11E-8 2.82E-9 8.79E-7 -2.44E-7
Potential soil quality index [-] 5.47E+3 1.73E+1 5.69E+1 1.14E+0 5.54E+1 -1.00E+2
Disclaimer 1 – for the indicator “potential Human exposure efficiency relative to U235“.
This impact category deals mainly with the eventual impact of low dose ionizing radiation on human health of the
nuclear fuel cycle. It does not consider effects due to possible nuclear accidents, occupational exposure nor
radioactive waste disposal in underground facilities. Potential ionizing radiation from the soil, from radon and
some construction materials, is also not measured by this indicator.
Disclaimer 2 – for the indicators “abiotic depletion potential for fossil resources”, “abiotic depletion potential for
non-fossil resources”, “water (user) deprivation potential”, “deprivation-weighted water consumption”, “potential
comparative toxic unit for ecosystems”, “potential comparative toxic unit for humans - cancer effects”, “potential
comparative toxic unit for humans – non-cancer effects”, “potential soil quality index
The results of this environmental impact indicator shall be used with care as the uncertainties on these results are
high or as there is limited experience with the indicator.
6. LCA: Interpretation
The supply chain, i.e. the production of the purchased overall green house gas emissions. At the same time a
materials, causes the highest influence on all impact credit (D) of 12% is given to the next system, due to
categories and the primary energy. the use of electrical and thermal energy, gained in the
incineration processes for the product and the off-cut
Global Warming Potential material.
Looking at the GWP for the overall declared life cycle
phases, including production (A1-A3), transport (A4, Further impact categories
C2), installation (losses) (A5) and end-of-life (C3, D), The end-of-life scenarios have less influence on the
the production (A1-A3) contributes to 43%. other considered impact categories than on GWP. The
The production in the supply chain (A1) already main contribution of the considered life cycle phases is
contributes 38% to the total GWP value. Thus, every concentrated on modules A1-A3.
increase in the production yield directly improves the The energy consumption in the foaming step
environmental performance of the products. influences all impact categories; variations depend on
The foaming process (A3), which includes the the national grid mixes for electricity.
electrical and thermal energy for the mixing, the
vulcanisation and blowing step as well as the Primary Energy Demand
production of the packaging materials, shows a The total primary energy demand is for both categories
significant influence on GWP of the life cycle with 5%. (renewable and non-renewable) significantly (> 100%)
Module A5 covers the production and disposal influenced by the production of the modules A1-A3.
(=incineration) of the off-cut material assumed as 1% The other modules play a minor role (C3 with about
loss in respect to the required insulation material. 6%)
Additionally, the emissions of the incineration of
packaging material (plastic, wood) in a waste The share of primary energy bound as material
incineration plant are considered. The installation step accounts for about 20%, which is partly recovered and
contributes with 25% to the overall GWP. credited for in module D (-16%)
As end-of-life scenario, incineration is considered. The
emissions of the product (C3) contribute to 42% of the
7. Requisite evidence
with FEF products (in living rooms) and
7.1 VOC emissions recommendation of the experts of the test institute, all
Eurofins Product Testing A/S has tested a wide range results were clearly below the limit values. For
and varieties of typical FEF (Flexible Elastomeric example the determined total volatile organic
Foam) products marketed in the EU from CEFEP compound (TVOC) after 28 days was for all samples
(European Group of FEF manufacturers). Sampling, below 100 mg/m3. Certificates are available on
testing and evaluation were performed according to request.
CEN TS 16516, AgBB, ISO 16000-3, ISO 16000-6,
ISO 16000-9, ISO 16000-11 in the latest versions. 7.2 Leaching performance
Based on the loading factor 0.2 m²/m³, which were According to EN 13468 is the content of water-soluble
determined after consideration of real life applications
9 Environmental Product Declaration Armacell GmbH – AF/ArmaFlex Evo insulation for industrial and building installation
chloride ions for AF/Armaflex ≤ 300 ppm.
8. References
AgBB EN 14706
Umweltbundesamt Germany, Health-related EN 14706: 2013-01: Thermal insulating products for
Evaluation of Emissions of Volatile Organic building equipment and industrial installations -
Compounds (VVOC, VOC and SVOC) from Building Determination of maximum service temperature
Products
EN 14707
CEFEP EN 14707: 2013-01: Thermal insulating products for
The industry association for FEF and PEF insulation building equipment and industrial installations -
(Celle) in 2012 Determination of maximum service temperature for
preformed pipe insulation
CEN TS 16516
CEN TS 16516:2013-12: Construction products - EN 15801
Assessment of release of dangerous substances - EN 15801: 2010-04: Conservation of cultural property -
Determination of emissions into indoor air Test methods - Determination of water absorption by
capillarity
Comission Decision 2001/118/EC
Amendment to European Waste Catalogue EN 15804
EN 15804:2019+A2, Sustainability of construction
CPR works — Environmental Product Declarations — Core
Regulation (EC) No 305/2011, Construction Products rules for the product category of construction products.
Regulation
EN 29052
EN 826 EN 29052: 1992-08: Acoustics; determination of
EN 826: 2013-05: Thermal insulating products for dynamic stiffness; part 1: materials used under floating
building applications - Determination of compression floors in dwellings
behaviour
EU/EFTA
EN 1606 Regulation (EU) No. 305/2011 (CPR), European
EN 1606: 2013-05: Thermal insulating products for Union/European Free Trade Association (EU/EFTA)
building applications - Determination of compressive
creep Eurofins Product Testing A/S
Eurofins Miljo, Smedeskowej 38, 8464 Galten,
EN 12091 Denmark
EN 12091: 2013-06: Thermal insulating products for
building applications - Determination of freeze-thaw European Waste Catalogue
resistance European Waste Catalogue and Hazardous Waste
List, Commission Decision 2000/532/EC
EN 12086
EN 12086:2013-06: Thermal insulating products for GaBi
building applications - Determination of water vapour GaBi 9 software-system and databases, LBP,
transmission properties University of Stuttgart and Sphera, Leinfelden-
Echterdingen, 2020 (http://documentation.gabi-
EN 13468 software.com/)
EN 13468: 2001-12: Thermal insulating products for
building equipment and industrial installations - IBU 2021
Determination of trace quantities of water soluble General Instructions for the EPD programme of Institut
chloride, fluoride, silicate, and sodium ions and pH Bauen und Umwelt e.V. Version 2.0, Berlin: Institut
Bauen und Umwelt e.V., 2021. www.ibu-epd.com
EN 13469
EN 13469:2013-01: Thermal insulating products for IBU PCR Part A
building equipment and industrial installations - PCR - Part A: Calculation Rules for the Life Cycle
Determination of water vapour transmission properties Assessment and Requirements on the Project Report,
of preformed pipe insulation Institut Bauen und Umwelt e.V., www.ibu-epd.com,
2019.
EN 13501-1
EN 13501-1: 2010-01: Fire classification of IBU PCR PART B
construction products and building elements - Part 1: PCR – Part B: Requirements on the EPD for Insulation
Classification using data from reaction to fire tests materials made of foam plastics, version 1.7, 01-2019 ,
Institut Bauen und Umwelt e.V., www.ibu-epd.com,
EN 14304 2019
EN 14304:2013-04: Thermal insulation products for
building equipment and industrial installations – ISO 3822-1
Factory made flexible elastomeric foam (FEF) products ISO 3822-1: 1999-05: Acoustics - Laboratory tests on
– Specification noise emission from appliances and equipment used in
10 Environmental Product Declaration Armacell GmbH – AF/ArmaFlex Evo insulation for industrial and building installation
water supply installations - Part 1: Method of compounds from building products and furnishing -
measurement Sampling, storage of samples and preparation of test
specimens
ISO 9001
ISO 9001:2014-08: Quality management systems – ISO 16000-3
Requirements ISO 16000-3:2011-10: Determination of formaldehyde
and other carbonyl compounds in indoor air and test
ISO 11654 chamber air - Active sampling method
ISO 11654: 1997-04: Acoustics - Sound absorbers for
use in buildings - Rating of sound absorption ISO 16000-6
ISO 16000-6:2011-12: Indoor air - Part 6:
ISO 14001 Determination of volatile organic compounds in indoor
ISO 14001:2015, Environmental management systems and test chamber air by active sampling on Tenax TA®
— Requirements with guidance for use sorbent, thermal desorption and gas chromatography
using MS or MS-FID
ISO 14025
ISO 14025:2011-10, Environmental labels and ISO 16000-9
declarations — Type III environmental declarations — ISO 16000-9:2006-02: Indoor air - Part 9:
Principles and procedures. Determination of the emission of volatile organic
compounds from building products and furnishing -
ISO 14040 Emission test chamber method
ISO 14040:2009-11: Environmental management –
Life cycle assessment – Principles and framework
REACH
ISO 14044 Regulation (EC) No 1907/2006, Regulation concerning
ISO 14044:2006-10: Environmental management – the Registration, Evaluation, Authorisation and
Life cycle assessment – Requirements and guidelines Restriction of Chemicals (REACH)
ISO 15868
ISO 15686:2011-05, Buildings and constructed assets
- Service life planning
ISO 16000-11
ISO 16000-11: 2006-02: Indoor air - Part 11:
Determination of the emission of volatile organic
11 Environmental Product Declaration Armacell GmbH – AF/ArmaFlex Evo insulation for industrial and building installation
Publisher
Institut Bauen und Umwelt e.V. Tel +49 (0)30 3087748- 0
Panoramastr. 1 Fax +49 (0)30 3087748- 29
10178 Berlin Mail info@ibu-epd.com
Germany Web www.ibu-epd.com
Programme holder
Institut Bauen und Umwelt e.V. Tel +49 (0)30 - 3087748- 0
Panoramastr 1 Fax +49 (0)30 – 3087748 - 29
10178 Berlin Mail info@ibu-epd.com
Germany Web www.ibu-epd.com
Author of the Life Cycle
Assessment Tel +49 711 341817-0
Sphera Solutions GmbH Fax +49 711 341817-25
Hauptstraße 111- 113 Mail info@sphera.com
70771 Leinfelden-Echterdingen Web http://www.sphera.com
Germany
Owner of the Declaration
Armacell International S.A. Tel +49-251-7603-0
Robert-Bosch-Str. 10 Fax +49-251-7603-346
48153 Münster Mail info.de@armacell.com
Germany Web www.armacell.de
