ENVIRONMENTAL PRODUCT DECLARATION
as per ISO 14025 and EN 15804+A2
Owner of the Declaration HALTON FOODSERVICE
Publisher Institut Bauen und Umwelt e.V. (IBU)
Programme holder Institut Bauen und Umwelt e.V. (IBU)
Declaration number EPD-HAL-20240072-IBA1-EN
Issue date 27/08/2024
Valid to 26/08/2029
CMW-I/FMOD - Cold Mist on Demand hood
HALTON FOOD SERVICE
www.ibu-epd.com | https://epd-online.com
1. General Information
HALTON FOOD SERVICE CMW-I/FMOD - Cold Mist on Demand hood
Programme holder Owner of the declaration
IBU – Institut Bauen und Umwelt e.V. HALTON FOODSERVICE
Hegelplatz 1 Zone Technoparc Futura CS 80102
10117 Berlin 62402 BETHUNE Cedex
Germany France
Declaration number Declared product / declared unit
EPD-HAL-20240072-IBA1-EN 1 linear metre of CMW-FMOD hood, used to extract heat and cooking
steam for 365 days a year, for 8 hours a day, for 15 years
This declaration is based on the product category rules: Scope:
Ventilation systems for commercial kitchens, 24/01/2024 This document refers to CMW-FMOD hood produced by HALTON
(PCR checked and approved by the SVR) FOODSERVICE in France. This EPD represents the declaration of a
specific product CMW-FMOD Hood, with the declared unit of 1 linear metre
of hood, used to extract heat and cooking steam for 365 days a year, for 8
Issue date hours a day, for 15 years.
The data collection for the ecological assessment occurred plant specific
27/08/2024
with current annual data. Consequently, the Life Cycle Assessment is
representative for this product.
The owner of the declaration shall be liable for the underlying information
Valid to
and evidence; the IBU shall not be liable with respect to manufacturer
26/08/2029 information, life cycle assessment data and evidences.
The EPD was created according to the specifications of EN 15804+A2. In
the following, the standard will be simplified as EN 15804.
Verification
The standard EN 15804 serves as the core PCR
Independent verification of the declaration and data according to ISO
14025:2011
internally X externally
Dipl.-Ing. Hans Peters
(Chairman of Institut Bauen und Umwelt e.V.)
Florian Pronold Dr. Matthew Fishwick,
(Managing Director Institut Bauen und Umwelt e.V.) (Independent verifier)
1 Environmental Product Declaration - HALTON FOOD SERVICE - CMW-I/FMOD - Cold Mist on Demand hood
2. Product
Biocide products were added to this construction product or it
2.1 Product description/Product definition has been treated with biocide products (this then concerns a
The Cold Mist on Demand and Water Wash hood (CMW- treated product as defined by the (EU) Ordinance on Biocide
I/FMOD) specializes in heavy duty and solid fuel appliances. Products No. 528/2012): no.
Different Halton sensors (Such as Thermal Imaging Matrix, Air
temperature, and Indoor Environment Quality) detect the 2.6 Manufacture
cooking activity of the appliance to determine its status and Manufacturing and packaging of the CMW-I/FMOD hood at the
activate the Cold Mist accordingly. production site. In this case, manufacturing mainly refers to the
Cold Mist technology is based on the use of a continuous, full- assembling, configuring, and testing of the hoods from pre-
length fine Cold Water Mist inside the exhaust plenum of the made parts. The assessment covers the electricity, LPG
hood to reduce the temperature of the air, neutralize the consumption for forklifts and water use needed during the
potential sparks and remove the grease from the exhausted air. production process. The electricity is modelled as site-specific
The Water Wash technology automatically washes down energy mixes provided by local energy companies.The waste
grease filters without the need for staff intervention. streams from the manufacturing site include, wastewater, wood
waste, cardboard, plastic and metal scrap (stainless steel and
The Capture Jet™ relates to the association of two sets of galvanised steel sheets).
nozzles supplied with an extremely low supply air volume (a Any production waste generated is disposed of according by
maximum of 30 m³/h/m of hood). Halton's waste contractor.
These nozzles fit to the lower part of the hood front as well as
the sides, encircling the perimeter of the covered cooking 2.7 Environment and health during manufacturing
areas. Workplace and emission limits are regularly monitored and are
The horizontal nozzles increase the push/pull of the thermal far below the prescribed limits.
plume and smoke from the lower part of the hood front due to
2.8 Product processing/Installation
the Venturi effect.
It provides an assist to push vapors back towards the filters. For The hood is installed in about 10 hours by 2 employees. The
the placing on the market of the product in the European hood is fixed by hand to the ceiling with the help of a lifter and
Union/European Free Trade Association (EU/EFTA) (with the some fixation devices.
exception of Switzerland) Regulation (EU) No. 305/2011 (CPR)
2.9 Packaging
applies. The product needs a declaration of performance taking
For product protection the hoods are individually packed in a
into consideration EN and the CE-marking.
cardboard box. All packaged products are wrapped with (low
For the application and use the respective national provisions
density polyethylene) PEBD/LDPE film on a wood pallet.
apply.
2.10 Condition of use
2.2 Application
To ensure the longevity of the product, a weekly cleaning (using
The CMW-I/FMOD hood is used for professional kitchens. They
water with 1.5% soap) and annual check-up on different hood
can be installed above the cooking appliances and is used to
parameters (Capture jets state, lighting state, filters (state and
remove fumes, odors, heat, humidity, and any airborne grease
number), k factor, exhaust rates in intake rates) are
from the environment.
recommended.
2.3 Technical Data
2.11 Environment and health during use
The technical properties are project-dependent (Airflow range).
The products do not emit any contaminants or substances that
The dimensions of the reference product is specified in the
are harmful to the environment or health during the use phase.
table below.
2.12 Reference service life
The service life is validated if the hood is installed following the
Constructional Data installation procedure. Reference service life for the cooker
Name Value Unit hoods is assumed 15 years.
The reference service life is based on the empirical value for
Length 1000 mm
the hoods when used in accordance with the care instructions.
Width 1400 mm
Height 500 mm 2.13 Extraordinary effects
Weight 125 kg Fire
power consumption (operation) 134 W The products are not classified as building materials (building
products) and are not subject to DIN 4102 and EN 13501-1.
Performance data of the product with respect to its Water
characteristics in accordance with the relevant technical No water-hazardous, toxic substances are washed-out to the
provision (no CE-marking). environment and water.
2.4 Delivery status
Mechanical destruction
The products vary in size as they are not catalogue products.
There are no relevant environmental impacts associated with
mechanical destruction.
2.5 Base materials/Ancillary materials
This product/article/at least one partial article contains other 2.14 Re-use phase
Carcinogenic, mutagenic, reprotoxic (CMR) substances in
The CMW-I/FMOD are not taken back by the manufacturer for
categories 1A or 1B which are not on the candidate list,
the purpose of reuse. Users can disassemble the products
exceeding 0.1 percentage by mass: no.
repeatedly within the reference utilization period and reuse it
elsewhere.
2 Environmental Product Declaration - HALTON FOOD SERVICE - CMW-I/FMOD - Cold Mist on Demand hood
2.15 Disposal 2.16 Further information
Disassembly of the products consists of the same steps as Additional information about our products can be found on
assembly, in reverse order. The product falls under the Waste Halton-website: www.halton.com.
from Electrical and Electronic Equipment (WEEE).
3. LCA: Calculation rules
or in water during use. Only the CMW-F model releases
3.1 Declared Unit detergent into the water. This detergent is certified Ecolab by
The declared unit is: '1 linear metre of hood, used to extract the Swan ecolabel. Phosphate-, NTA-, EDTA- and chlorine-free.
heat and cooking steam for 365 days a year, for 8 hours a day, This impact is therefore negligible.
for 15 years'.
Declared unit Module B2:
- a weekly cleaning with 5L of water containing 1,5% soap.
Name Value Unit
- annual check-up by a technician on different hood parameters
Declared unit 1 rm
(Capture jets state, lighting state, filters (state and number), k
Mass per Unit 125 kg factor, exhaust rates in intake rates) modelled with
linear density 125 kg/rm transportation of one technician in light commercial vehicle (100
km). The number of check-ups depends on the hood model.
Other declared units are allowed if the conversion is shown
- 2 UV light replacements during the reference life service.
transparently.
- End-of-life treatment of 2 UV light tubes during SLR with
transportation included
3.2 System boundary
Module B6 et B7
This representative EPD follows the EPD type "cradle to grave".
The hood is designed for heavy duty industrial usage. To reflect
The following life cycle modules are declared:
the most average scenario the hood will be functioning 8 hours
a days 7 days a week. Electricity (B6) and water (B7) are
Modules A1-A3
required to use the products.
The product stage begins with considering the production of the
necessary raw materials (metals, electronics, packaging
Modules C1-C4
materials), including all corresponding upstream chains and the
The module includes the environmental impacts for dismantling
actual procurement transports.
of the products and the treatment of the CMW-I/FMOD hood
Furthermore, the entire manufacturing phase was mapped,
waste until the end-of-waste status (EoW) is reached, including
including the treatment of production waste until the end-of
the associated transports at the end of the product life cycle.
waste status (EoW) was reached.
The product is assumed to be removed manually at the same
time as the building is demolished. No scenario has been
Module A4
developed for stage C1.
The transport model considers a construction site in Europe.
The scenario for the distribution stage considers a average
The hood and the ceiling beam are removed separately.
distance by truck to serve the entire European area from the
Dismantling of product components at recycling facility. Based
Halton's plant. The quantity transported corresponds to the
on the material, components are either recycled, incinerated, or
transport of products and their packaging to the construction
landfilled depending on the material.
site.
Stage C3 represents the impact of a conventional scrap
Module A5
processing site, with sorting, shearing, shredding, separation.
The hood is delivered at the right size on the installation site. It
is installed in about 10 hours by 2 employees. The hood is fixed
Module D
to the ceiling with the help of a lifter and some fixation devices.
Identification of the benefits and costs of the product outside
the system boundary.
Complementary products for installation include a ceiling beam
Recycling of metal scrap results in credits of the respective raw
in galvanised steel. This additional product is supplied by
materials for the primary material portion of the input. The loads
Halton. Their production and packaging are considered in A1,
of the waste incineration and recycling processes are assigned
their transport in A3 and A4 and the end-of-life of their
to the respective modules (A3, A5 and C3) and not to module
packaging in A5.
D.
Others complementary products are used to fix the MUPRO
Ceiling beam (clip, pin, screw). They must be purchased by the
3.3 Estimates and assumptions
installer because they depend on ceiling type (metallic,
Energy and water consumption during production could only be
concrete or wood). They are not considered in this study.
determined on existing products and not on the average
product.
The application phase considers:
- Transportation of material lifter to installation site 3.4 Cut-off criteria
- Waste treatment (product packaging)
Cut-off criteria follow EN15804 and PCR Part A. No flows have
been deliberately omitted from the system boundaries.
Modules B1 & B3-B5 & B7
These modules were considered but evaluated as not relevant 3.5 Background data
for the products and considered as zero. Products do not All background data was considered using data from the
require repair (B3)/replacement (B4)/rehabilitation (B5). Ecoinvent 3.7.1 database or literary sources.
The hoods haven't significant impact for emission in indoor air 3.6 Data quality
3 Environmental Product Declaration - HALTON FOOD SERVICE - CMW-I/FMOD - Cold Mist on Demand hood
Site-specific production data has been collected for 2021 from energy use, where allocation could not be avoided, the
the production site. The upstream and downstream processes consumption of electricity and water in Halton's plant were
have been modelled based on environmental data from generic allocated per working hours for assembly of each product. No
databases ecoinvent. The collected data was reviewed in terms other allocations were made in this assessment. The cut-off
of consistency, and it is estimated as good quality. end-of-life allocation approach was used throughout.
3.7 Period under review 3.10 Comparability
The data is therefore based on 2021. All information is based Basically, a comparison or an evaluation of EPD data is only
on averaged data for 12 consecutive months. possible if all the data sets to be compared were created
according to EN 15804 and the building context, respectively
3.8 Geographic Representativeness the product-specific characteristics of performance, are taken
Land or region, in which the declared product system is into account. According to the EN 15804 standard,
manufactured, used or handled at the end of the product´s environmental declarations for construction products may not
lifespan: Europe be comparable if they have not been prepared in accordance
with that standard or if a different notified unit has been
used.The LCA was conducted using SimaPro 9.2.0.2. software.
3.9 Allocation
All background data was considered using data from the
Allocation has been avoided whenever possible by collecting
ecoinvent 3.7.1 (cut-off) database or literary sources.
product specific environmental data. In case of manufacturing
4. LCA: Scenarios and additional technical information
without energy recovery, 22% landfill.
Characteristic product properties of biogenic carbon
The biogenic carbon content quantifies the amount of biogenic NHW
carbon in a construction product leaving the factory gate, and it Cardboard: 4.33E+00 kg → 82% recycling, 9% incineration
shall be separately declared for the product and for any without energyrecovery, 9% landfill.
accompanying packaging.
Maintenance (B2)
The mass of packaging containing biogenic carbon is declared.
Name Value Unit
Note: 1 kg of biogenic carbon is equivalent to 44/12 kg of CO . Total number of check-up
2 60 number
during SRL
Name Value Unit
Estimated distance for round
Biogenic carbon content of the product 0 kg.C 100 km
trip
Biogenic carbon content of associated packaging 15.2 kg.C
Estimated weight of
technician doing the check 80 kg
The scenarios and assumptions applied in this study for all the up.
life cycle stages included are based on data provided by Halton
2 replacements of UV light 5.40E-
and correspond to the most likely scenario. The following kg
during SLR 01
scenarios and general assumptions were made in the studied
3.09E m3 of water containing
lifecycle stages: Weekly cleaning
+03 1,5% soap /DVR
Transport (A4) Operational energy and water use (B6-B7)
All trucks used in transportation were assumed to be class Name Value Unit
EURO6 trucks.
Total consumption of electricity during one year 3.91E+02kWh
Name Value Unit Total consumption of water during one year 2.12E+05 kg
Transport of distance 1631.4 km
End of life (C1-C4)
Capacity utilization (including empty runs) ~19 %
Name Value Unit
Installation into the building (A5)
Transport to treatment site 50 km
Name Value Unit
The following end of life scenarios are considered for the
Material loss 0 %
product:
The
following end of life scenarios are considered for packaging: NHW Plastic: 1.27E+00 kg → 41% recycling, 37% incineration
without energy recovery, 22% landfill
NHW NHW Steel: 1.16E+02 kg → 90% recycling, 10% landfill NHW
Wood: 3.00E+01 kg → 31% recycling, 31% incineration without Glass: 6.97E-01 kg → 100% landfill
energy recovery, 38% landfill. NHW WEE: 7.63E+00 kg → 74.7% recycling, 1.8% reuse, 9.7%
incineration without energy recovery, 13.8% landfill
NHW
Plastic: 1.43E+00 kg → 41% recycling, 37% incineration Life Span according to the manufacturer is 15 years.
4 Environmental Product Declaration - HALTON FOOD SERVICE - CMW-I/FMOD - Cold Mist on Demand hood
5. LCA: Results
The following table shows the result of the LCA for 1 m of a CMW-I/FMOD hood.
DESCRIPTION OF THE SYSTEM BOUNDARY (X = INCLUDED IN LCA; MND = MODULE OR INDICATOR NOT DECLARED; MNR
= MODULE NOT RELEVANT)
Benefits and
Construction loads beyond
Product stage Use stage End of life stage
process stage the system
boundaries
la ire ta m w a Ry lp p u s tro p s n a rT g n iru tc a fu n a M e h t m o rf tro p s n a rTe tis e h t o t e ta g y lb m e s s A e s U e c n a n e tn ia M ria p e R tn e m e c a lp e R tn e m h s ib ru fe R y g re n e la n o ita re p Oe s u re ta w la n o ita re p Oe s u n o itc u rts n o c -e Dn o itilo m e d tro p s n a rT g n is s e c o rp e ts a W la s o p s iD -e s u e R-y re v o c e R-g n ilc y c e Rla itn e to p
A1 A2 A3 A4 A5 B1 B2 B3 B4 B5 B6 B7 C1 C2 C3 C4 D
X X X X X MND X MNR MNR MNR X X X X X X X
RESULTS OF THE LCA - ENVIRONMENTAL IMPACT according to EN 15804+A2: 1 m CMW-I/FMOD hood
Parameter Unit A1-A3 A4 A5 B2 B6 B7 C1 C2 C3 C4 D
GWP-total kg CO 2 eq 1.79E+03 3.34E+01 1.14E+02 1.44E+03 2.46E+03 1.09E+03 0 1.02E+00 3.12E+00 3.76E+00 -1.76E+02
GWP-fossil kg CO 2 eq 1.83E+03 3.34E+01 4.6E+01 1.27E+03 2.44E+03 1.09E+03 0 1.02E+00 1.11E+00 3.28E+00 -1.76E+02
GWP-
biogenic kg CO 2 eq -4.71E+01 1.29E-02 6.8E+01 2.1E+01 1.41E+01 4.46E+00 0 3.92E-04 2.01E+00 4.76E-01 -3.37E-01
GWP-luluc kg CO 2 eq 2.4E+00 1.14E-02 2.17E-02 1.45E+02 5.06E+00 1.58E+00 0 3.49E-04 8.55E-04 6.74E-05 -7.26E-02
kg CFC11
ODP 1.12E-04 7.59E-06 8.64E-06 2.09E-04 1.24E-04 7.29E-05 0 2.31E-07 1.69E-07 4.63E-08 -6.91E-06
eq
AP mol H+ eq 1.1E+01 9.28E-02 1.55E-01 7.41E+00 1.33E+01 5.96E+00 0 2.83E-03 8.63E-03 1.66E-03 -6.39E-01
EP-
kg P eq 1.74E-01 2.5E-04 4.88E-04 7.82E-01 2.59E-01 8.54E-02 0 7.63E-06 7.19E-05 7.58E-06 -8.74E-03
freshwater
EP-marine kg N eq 2.1E+00 1.89E-02 5.78E-02 3.03E+00 1.78E+00 9.84E-01 0 5.76E-04 4.51E-03 1.15E-03 -1.5E-01
EP-terrestrial mol N eq 2.33E+01 2.1E-01 4.75E-01 2.4E+01 2.04E+01 1.1E+01 0 6.41E-03 3.16E-02 7.02E-03 -1.62E+00
kg NMVOC
POCP 6.44E+00 8.05E-02 1.51E-01 6.91E+00 5.57E+00 3.57E+00 0 2.46E-03 7.95E-03 2.04E-03 -8.01E-01
eq
ADPE kg Sb eq 2.35E-01 1.23E-04 2.61E-04 2.5E-02 2.22E-02 5.41E-03 0 3.74E-06 7.12E-05 5.71E-07 -2.48E-04
ADPF MJ 2.37E+04 5.06E+02 6.03E+02 1.79E+04 5.16E+04 1.88E+04 0 1.54E+01 1.07E+01 2.8E+00 -1.74E+03
m3 world eq
WDP 5.56E+02 1.46E+00 2.29E+00 7.67E+02 5.29E+02 1.37E+05 0 4.46E-02 -5.11E-02 1.91E-01 1.41E+00
deprived
GWP = Global warming potential; ODP = Depletion potential of the stratospheric ozone layer; AP = Acidification potential of land and water; EP =
Eutrophication potential; POCP = Formation potential of tropospheric ozone photochemical oxidants; ADPE = Abiotic depletion potential for non-fossil
resources; ADPF = Abiotic depletion potential for fossil resources; WDP = Water (user) deprivation potential)
RESULTS OF THE LCA - INDICATORS TO DESCRIBE RESOURCE USE according to EN 15804+A2: 1 m CMW-I/FMOD hood
Parameter Unit A1-A3 A4 A5 B2 B6 B7 C1 C2 C3 C4 D
PERE MJ 3.95E+03 6.91E+00 1.26E+01 2.13E+03 9.29E+03 2.31E+03 0 2.11E-01 2.11E+00 6.87E-02 -2.39E+02
PERM MJ 5.65E+02 0 -2.15E+02 0 0 0 0 0 0 0 0
PERT MJ 4.51E+03 6.91E+00 -2.03E+02 2.13E+03 9.29E+03 2.31E+03 0 2.11E-01 2.11E+00 6.87E-02 -2.39E+02
PENRE MJ 2.35E+04 5.06E+02 6.28E+02 1.81E+04 5.08E+04 1.86E+04 0 1.54E+01 1.06E+01 2.8E+00 -1.73E+03
PENRM MJ 1.34E+02 0 -2.52E+01 0 0 0 0 0 0 -4.79E+00 0
PENRT MJ 2.36E+04 5.06E+02 6.02E+02 1.8E+04 5.07E+04 1.86E+04 0 1.54E+01 1.05E+01 -1.99E+00 -1.73E+03
SM kg 0 0 0 0 0 0 0 0 0 0 0
RSF MJ 0 0 0 0 0 0 0 0 0 0 0
NRSF MJ 0 0 0 0 0 0 0 0 0 0 0
FW m3 2.38E+01 6.92E-02 1.19E-01 2.64E+01 4.26E+01 3.2E+03 0 2.11E-03 4.65E-03 5.34E-03 -1.33E-01
PERE = Use of renewable primary energy excluding renewable primary energy resources used as raw materials; PERM = Use of renewable primary
energy resources used as raw materials; PERT = Total use of renewable primary energy resources; PENRE = Use of non-renewable primary energy
excluding non-renewable primary energy resources used as raw materials; PENRM = Use of non-renewable primary energy resources used as raw
materials; PENRT = Total use of non-renewable primary energy resources; SM = Use of secondary material; RSF = Use of renewable secondary fuels;
NRSF = Use of non-renewable secondary fuels; FW = Use of net fresh water
RESULTS OF THE LCA – WASTE CATEGORIES AND OUTPUT FLOWS according to EN 15804+A2:
1 m CMW-I/FMOD hood
Parameter Unit A1-A3 A4 A5 B2 B6 B7 C1 C2 C3 C4 D
HWD kg 7.56E+02 3.48E-01 3.31E+00 7.39E+01 5.7E+01 7.14E+01 0 1.06E-02 5.78E-01 1.98E-01 -1.76E+01
NHWD kg 2.42E+03 2.88E+01 3.8E+01 9.98E+02 9.32E+02 9.8E+02 0 8.79E-01 2.71E+00 1.18E+01 -4.15E+02
RWD kg 8.2E-02 3.46E-03 4.02E-03 1.03E-01 3.63E-01 1.09E-01 0 1.06E-04 1.21E-04 1.56E-05 -2.94E-03
CRU kg 0 0 0 7.39E+01 5.7E+01 7.14E+01 0 0 5.78E-01 0 -1.76E+01
MFR kg 4.26E+01 0 1.34E+01 9.98E+02 9.32E+02 9.8E+02 0 0 2.71E+00 0 -4.15E+02
MER kg 0 0 0 1.03E-01 3.63E-01 1.09E-01 0 0 1.21E-04 0 -2.94E-03
EEE MJ 0 0 0 0 0 0 0 0 1.37E-01 0 0
5 Environmental Product Declaration - HALTON FOOD SERVICE - CMW-I/FMOD - Cold Mist on Demand hood
EET MJ 0 0 0 0 0 0 0 0 0 0 0
HWD = Hazardous waste disposed; NHWD = Non-hazardous waste disposed; RWD = Radioactive waste disposed; CRU = Components for re-use;
MFR = Materials for recycling; MER = Materials for energy recovery; EEE = Exported electrical energy; EET = Exported thermal energy
RESULTS OF THE LCA – additional impact categories according to EN 15804+A2-optional:
1 m CMW-I/FMOD hood
Parameter Unit A1-A3 A4 A5 B2 B6 B7 C1 C2 C3 C4 D
Disease
PM 1.12E-04 2.1E-06 2.11E-06 1.19E-04 3.52E-05 4.94E-05 0 6.41E-08 1.37E-07 3.15E-08 -1.11E-05
incidence
IR kBq U235 eq 9.49E+01 2.22E+00 2.66E+00 7.82E+01 4.46E+02 1.29E+02 0 6.79E-02 1.08E-01 1.05E-02 -2.68E+00
ETP-fw CTUe 8.87E+04 3.89E+02 5.97E+02 3.55E+04 3.22E+04 1.83E+04 0 1.19E+01 2.93E+02 7.09E+01 -4.18E+03
HTP-c CTUh 1.52E-05 1.38E-08 2.54E-08 1.97E-06 9.6E-07 4.42E-06 0 4.21E-10 2.64E-09 1.14E-09 -1.07E-06
HTP-nc CTUh 4.81E-05 3.8E-07 5.5E-07 2.23E-05 2.53E-05 6.1E-05 0 1.16E-08 4.89E-08 1.4E-08 -3.68E-06
SQP SQP 2.68E+04 5.18E+02 4.24E+02 3.12E+04 1.66E+04 7.58E+03 0 1.58E+01 1.17E+02 4.5E+00 -2.37E+03
PM = Potential incidence of disease due to PM emissions; IR = Potential Human exposure efficiency relative to U235; ETP-fw = Potential comparative
Toxic Unit for ecosystems; HTP-c = Potential comparative Toxic Unit for humans (cancerogenic); HTP-nc = Potential comparative Toxic Unit for humans
(not cancerogenic); SQP = Potential soil quality index
Disclaimer 1 – for the indicator “Potential Human exposure efficiency relative to U235”. This impact category deals mainly with the
eventual impact of low-dose ionizing radiation on human health of the nuclear fuel cycle. It does not consider effects due to possible
nuclear accidents, occupational exposure or radioactive waste disposal in underground facilities. Potential ionizing radiation from the
soil, radon and from some construction materials is also not measured by this indicator.
Disclaimer 2 – for the indicators “abiotic depletion potential for non-fossil resources”, “abiotic depletion potential for fossil resources”,
“water (user) deprivation potential, deprivation-weighted water consumption”, “potential comparative toxic unit for ecosystems”,
“potential comparative toxic unit for humans – cancerogenic”, “Potential comparative toxic unit for humans - not cancerogenic”,
“potential soil quality index”. The results of this environmental impact indicator shall be used with care as the uncertainties on these
results are high as there is limited experience with the indicator.
6. LCA: Interpretation
The dominance analysis shows that modules B2, B6 and A1
are the dominant life cycle stages in most of the categories.
The contribution of B2 is due to the transportation of a
technician for an annual check-up. Module B6 dominates most
indicators due the electricity energy demand for using. B7 has a
high contribution to water use due to water consumption during
service life. The modules A1-A3 have great contributions to all
categories especially for the Depletion of abiotic resources -
minerals and metals. In this indicator the provision of chromium
steel has the largest contribution. The end-of-life stage has no
significant influence on the environmental indicators. The
environmental burdens from the transports (modules A4 and
C2) account for 1% of the total burdens from the transports in
all cases.
7. Requisite evidence
8. References
PCR 2020, Part A EN 15804
Institut Bauen und Umwelt e.V., Berlin (pub.): Product EN 15804:2012+A2:2019+AC:2021, Sustainability of
Category Rule for Construction Products from the construction works — Environmental Prouct Declarations —
range of Environmental Product Declarations of Core rules for the product category of construction products.
Institute Bauen und Umwelt (IBU), Part A: Calculation
rules for the Life Cycle Assessment and requirements ISO 14025
on the project report according to EN 15804+A2. EN ISO 14025:2011, Environmental labels and declarations —
Version 2020-07. Type III environmental declarations — Principles and
www.ibu-epd.com procedures.
PCR 2024, Part B DIN 4102-1
Product Category Rules for Construction Products, DIN 4102-1: Fire behaviour of building materials andbuilding
Part B: Ventilations systems for commercial kitchens, components - Part 1: Building materials;concepts, requirements
24/01/2024 and tests. 1998-05
6 Environmental Product Declaration - HALTON FOOD SERVICE - CMW-I/FMOD - Cold Mist on Demand hood
DIN EN 13501-1 Commission Directives 91/155/EEC, 93/67/EEC,
DIN EN 13501-1:2019-05: Fire classification ofconstruction 93/105/EC and 2000/21/EC, 2006-12.
products and building elements - Part 1:Classification using
data from reaction to fire tests;German version EN 13501- Biocide Guideline
1:2018 Regulation (EU) No. 528/2012 of the European
Parliament and of the Council of 22 May 2012
concerning the making available on the market and
/Further References use of biocidal products
SimaPro 9.2.0.2 CPR
Directive (EU) No. 305/2011 of the European
WEEE Parliament and Council dated 9 March 2011
Waste Electrical and Electronic Equipment Directive : Act establishing harmonised conditions for marketing
governing the requirements on utilisation and disposal of construction products and replacing Council Guideline
WEEE. 89/106/EEC
Ecoinvent
REACH Regulation Ecoinvent database version 3.7.1
Regulation (EC) No. 1907/2006 of the European
Parliament and of the Council of 18 December 2006
concerning the Registration, Evaluation, Authorisation IBU 2021
and Restriction of Chemicals (REACH), establishing a Institut Bauen und Umwelt e.V.: General Instructions for the
European Chemicals Agency, amending Directive EPD programme of Institut Bauen und Umwelt e.V., Version
1999/45/EC and repealing Council Regulation (EEC) 2.0, Berlin: Institut Bauen und Umwelt e.V., 2021
No. 793/93, Commission Regulation (EC) No. 1488/94 www.ibu-epd.com
as well as Council Directive 76/769/EEC and
7 Environmental Product Declaration - HALTON FOOD SERVICE - CMW-I/FMOD - Cold Mist on Demand hood
Publisher
Institut Bauen und Umwelt e.V. +49 (0)30 3087748- 0
Hegelplatz 1 info@ibu-epd.com
10117 Berlin www.ibu-epd.com
Germany
Programme holder
Institut Bauen und Umwelt e.V. +49 (0)30 3087748- 0
Hegelplatz 1 info@ibu-epd.com
10117 Berlin www.ibu-epd.com
Germany
Author of the Life Cycle Assessment
CSTB 04 56 14 72 62
rue Joseph Fourier 24 cecile.magnin-feysot@cstb.fr
38400 Saint-Martin-d'Hères https://www.cstb.fr/fr/
France
Owner of the Declaration
HALTON FOODSERVICE 06.14.71.06.55
Zone Technoparc Futura CS 80102 arnaud.kazmierczak@halton.com
62402 BETHUNE Cedex https://www.halton.com/fr/
France
8 Environmental Product Declaration - HALTON FOOD SERVICE - CMW-I/FMOD - Cold Mist on Demand hood
