Environmental Product Declaration (EPD)
According to ISO 14025 and EN 15804
ACEGrid®
Registration number: EPD-Kiwa-EE-158054-EN
Issue date: 22-12-2023
Valid until: 22-12-2028
Declaration owner: Gold-Joint Industry Co., Ltd.
Publisher: Kiwa-Ecobility Experts
Program operator: Kiwa-Ecobility Experts
Status: verified
ACEGrid® | ReTHiNK-58054 1 / 25
Environmental Product Declaration
1 General information
E-mail: marketing@geoace.com
1.1 PRODUCT Website: www.geoace.com
Production location: Gold-Joint Industry Co., Ltd.
ACEGrid®
Address production location: No.33, Jing 3 Rd. Wuqi Dist., 43541 Taichung City
1.2 REGISTRATION NUMBER
1.6 VERIFICATION OF THE DECLARATION
EPD-Kiwa-EE-158054-EN
The independent verification is in accordance with the ISO 14025:2011. The LCA is in
1.3 VALIDITY compliance with ISO 14040:2006 and ISO 14044:2006. The EN 15804:2012+A2:2019 serves as
the core PCR.
Issue date: 22-12-2023
Internal ✓ External
Valid until: 22-12-2028
1.4 PROGRAM OPERATOR
Kiwa-Ecobility Experts
Voltastraße 5
13355 Berlin
DE
Elisabeth Amat Guasch, Greenize
1.7 STATEMENTS
Prof. Dr. Frank Heimbecher
The owner of this EPD shall be liable for the underlying information and evidence. The
(Chairman of the independent expert
programme operator Kiwa-Ecobility Experts shall not be liable with respect to
committee - Kiwa-Ecobility Experts)
manufacturer data, life cycle assessment data and evidence.
Frank Huppertz 1.8 PRODUCT CATEGORY RULES
(Head of Kiwa-Ecobility Experts)
Kiwa-Ecobility Experts (Kiwa-EE) – General Product Category Rules (2022-02-14)
Kiwa-Ecobility Experts (Kiwa-EE) – Specific Product Category Rules: Geosynthetic products
1.5 OWNER OF THE DECLARATION
(2023-07-21)
Manufacturer: Gold-Joint Industry Co., Ltd.
Address: No.33, Jing 3 Rd. Wuqi Dist., 43541 Taichung City, Taiwan (R.O.C.)
ACEGrid® | ReTHiNK-58054 2 / 25
Environmental Product Declaration
1 General information
1.9 COMPARABILITY 1.10 CALCULATION BASIS
In principle, a comparison or assessment of the environmental impacts of different LCA method R<THiNK: Ecobility Experts | EN15804+A2
products is only possible if they have been prepared in accordance with EN 15804. For the
evaluation of the comparability, the following aspects have to be considered in particular: LCA software*: Simapro 9.1
PCR used, functional or declared unit, geographical reference, the definition of the system Characterization method: EN 15804 +A2 Method v1.0
boundary, declared modules, data selection (primary or secondary data, background
database, data quality), scenarios used for use and disposal phases, and the life cycle LCA database profiles: EcoInvent version 3.6
inventory (data collection, calculation methods, allocations, validity period). PCRs and Version database: v3.15 (2023-07-12)
general program instructions of different EPDs programs may differ. Comparability needs
to be evaluated. For further guidance, see EN 15804+A2 (5.3 Comparability of EPD for
*Used for calculating the characterized results of the Environmental profiles within
construction products) and ISO 14025 (6.7.2 Requirements for comparability).
R<THiNK.
1.11 LCA BACKGROUND REPORT
This EPD is generated on the basis of the LCA background report 'ACEGrid®' with the
calculation identifier ReTHiNK-58054.
ACEGrid® | ReTHiNK-58054 3 / 25
Environmental Product Declaration
2 Product
2.1 PRODUCT DESCRIPTION
2.2 APPLICATION (INTENDED USE OF THE PRODUCT)
ACEGrid® represents a line of flexible, high-strength woven geogrids made from high
molecular weight, low-creep polyester (PET) yarns. The geogrids offer a wide range of
ACEGrid® geogrids, known for their commendable tensile strength and adaptability, are
tensile strengths, up to 1000 kN/m, to suit various soil reinforcement applications. The
considered for various applications within civil engineering. Their versatility has been
weight of the product is between 240 g/m² and 2600 g/m². Distinguished by their high
recognized for potential deployment across different terrains and functionalities.
tensile strength at low strain levels and anti-creep performance, these geogrids provide
durability against environmental conditions like UV light, weathering, and chemicals. For Mechanically Stabilized Earth Walls (MSEW) and Reinforced Soil Slopes (RSS),
Customizable to specific project requirements, ACEGrid® geogrids are effective in diverse ACEGrid® geogrids have been explored to provide a synergy between geogrid attributes
civil and transportation engineering projects worldwide. Renowned for their high quality, and backfill materials. These combined systems aim to offer both stability and flexibility.
long-term durability, and ease of installation, these geogrids are a cost-effective solution They're considered for diverse structures, including retaining walls, road embankments,
for long-term structural safety. bridge abutments, landfill embankments, sea walls, rockfall prevention embankments,
crusher headwalls and loading ramps, and flood detention ponds, among others.
The following products are covered in this EPD: GG40-I, GG60-I, GG80-I, GG100-I, GG110-I,
GG150-I, GG200-I, GG300-I, GG400-I, GG600-I, GG800-I, GG900-I, GG1000-I. In the realm of basal reinforcement, the inherent strength of ACEGrid® geogrids suggests
their potential in enhancing foundational structures. Their application might span
embankments on soft soil, reinforced embankment on piles, and reinforcement over
cavities.
Mining pits, which can sometimes face challenges like shifts or collapses, might benefit
from ACEGrid® geogrids when integrated appropriately. Their presence could potentially
bolster the site, adding a layer of protection and enhancing overall safety during mining
operations.
For energy infrastructure projects, ACEGrid® geogrids can support the construction of oil
and gas pipelines, wind farms, solar farms, and other energy infrastructure by providing
ground stabilization and reinforcement. Additionally, their integration could be beneficial
in safeguarding against landslides, especially during the installation and utilization of
landfill capping systems on challenging terrains.
In concluding, ACEGrid® geogrids offer promising options for various civil engineering
tasks. However, their effectiveness is best evaluated concerning the specific requirements
and conditions of each project.
2.3 REFERENCE SERVICE LIFE
RSL PRODUCT
The RSL of the geogrid depends on the use from a temporary work or a long-term use
(from 1 year to 120 years). For examples, geogrids used in road embankments have a typical
service life of 60 years. Geogrid used for retaining walls which have a typical service life of
120 years.
USED RSL (YR) IN THIS LCA CALCULATION:
120
ACEGrid® | ReTHiNK-58054 4 / 25
Environmental Product Declaration
2 Product
2.4 TECHNICAL DATA
See above (2.1).
2.5 SUBSTANCES OF VERY HIGH CONCERN
The product contains less than 0.1% of substances included in the “Candidate list of
substances of very high concern for authorisation” (SVHC).
2.6 DESCRIPTION PRODUCTION PROCESS
The production process of ACEGrid® geogrid begins with PET yarn as its fundamental
material. Prior to weaving, the original yarn is twisted into processed yarn, a task executed
by external partnering manufacturers. Upon completion, the processed yarn is transported
via truck back to the Gold-Joint factory.
The processed yarn is used directly for the ACEGrid® production line. The processed yarn is
placed on the creel for weaving.Weaving is a method of fabric production. Two different
sets of yarns are woven and interlaced at right angles, i.e. the longitudinal warp direction
(machine direction) and the transversal weft direction (cross machine di-reaction).
2.7 CONSTRUCTION DESCRIPTION
The finished mesh product of weaving, it is dipped in tank to coat the mesh with a
protective. After drying, the coated mesh is cut to specific length and stored, the outer The applications of ACEGrid® are extensive, generally include RSS, MSEW, bridge
packaging is done before shipment. abutment, embankment, etc. The ACEGrid® construction can be divided into the
following parts:
1. Site preparation
2. Geogrid installation
3. Backfill and compaction
4. Facing installation
5. Drainage system installation
6. Surface drainage and vegetation
ACEGrid® | ReTHiNK-58054 5 / 25
Environmental Product Declaration
2 Product
ACEGrid® | ReTHiNK-58054 6 / 25
Environmental Product Declaration
3 Calculation rules
3.1 DECLARED UNIT Module B2 = Maintenance Module C4 = Disposal
Module D = Benefits and loads beyond the
One square meter ACEGrid® Module B3 = Repair
product system boundaries
One square meter of ACEGrid®. The following products are covered in this EPD: GG40-I,
Module B4 = Replacement
GG60-I, GG80-I, GG100-I, GG110-I, GG150-I, GG200-I, GG300-I, GG400-I, GG600-I, GG800-I,
GG900-I, GG1000-I.
reference_unit: square meter (m2) 3.4 REPRESENTATIVENESS
The input data are representative for ACEGrid®, a product of Gold-Joint Industry Co., Ltd..
3.2 CONVERSION FACTORS
The data are representative for Asia.
Description Value Unit
3.5 CUT-OFF CRITERIA
reference_unit 1 m2
weight_per_reference_unit 1.000 kg Product Stage (A1-A3)
Conversion factor to 1 kg 0.999540 m2
The following inputs have been placed under cut-off criteria (<1% of the total mass):
3.3 SCOPE OF DECLARATION AND SYSTEM BOUNDARIES -Raw materials : Stabilizer, Disperser
-Ancillary materials : Release agent, Grease, Stain remover
This is a Cradle to gate with options, modules C1-C4 and module D LCA. The life cycle
stages included are as shown below:
Construction process stage (A4-A5)
(X = module included, ND = module not declared)
A1 A2 A3 A4 A5 B1 B2 B3 B4 B5 B6 B7 C1 C2 C3 C4 D This stage consists the transport of the product from production plant to the construction
X X X X X ND ND ND ND ND ND ND X X X X X site.
It also includes the loss of material during construction. The additional needed production,
transport and end-of-life of the lost material during construction is included.
The modules of the EN15804 contain the following:
The end-of-life of packaging material up to the end-of-waste state or disposal of final
Module A1 = Raw material supply Module B5 = Refurbishment residues is also included.
Module A2 = Transport Module B6 = Operational energy use
Module A3 = Manufacturing Module B7 = Operational water use End of life stage (C1-C4)
Module A4 = Transport Module C1 = De-construction / Demolition
Module A5 = Construction - When the end of the life stage of the building is reached, the de-construction/demolition
Module C2 = Transport begins. This EPD includes de-construction/demolition (C1), the necessary transport (C2)
Installation process from the demolition site to the sorting location and distance to final disposal. The end of
Module B1 = Use Module C3 = Waste Processing life stage includes the final disposal to landfill (C4), incineration (C3) and needed recycling
ACEGrid® | ReTHiNK-58054 7 / 25
Environmental Product Declaration
3 Calculation rules
processes up to the end-of-waste point (C3). Loads and benefits of recycling, re-use and
exported energy are part of module D. -Raw materials : Stabilizer, Disperser
The prescribed waste scenarios from the NMD Determination method v1.0 have been used -Ancillary materials : Release agent, Grease, Stain remover
for the various materials in the product.
A scaling method was used to calculate the LCA results for the different ACEGrid®
products. The scaling was done on the basis of mass per square meter. As a result of
Benefits and Loads beyond the system boundary (Module D) scaling there are results for both the fixed and the scalable part of the scaling function.
The fixed part means that this number is the same for each product in the product group
and the scalable part is the part that depends on the mass per unit area of the product. In
This stage contains the potential loads and benefits of recycling and re-use of raw order to calculate the correct number of each environmental impact category for each of
materials/products. The loads contain the needed recycling processes from end-of-waste- the products in the product group, the following calculation should be done:
point up to the point-of-equivalence of the substituted primary raw material and a load for
secondary material that will be lost at the end-of-life stage. [number fixed part]+([specific mass]*[number scalable part])
The loads and benefits of recycling and reuse are included in this module. The benefits are The inputs calcium carbonate and cardboard tube did not have a linear dependence on
calculated based on the primary content and the primary equivalent. the specific mass, so the higher amount of product available was always considered for
scaling to be as conservative as possible.
In addition, the benefits of energy recovery are granted at this stage. The amount of avoid
energy is based on the Lower Heating Values of the materials and the efficiencies of the The linear dependence of energy consumption on specific mass has been calculated by
incinerators as mentioned in the NMD Determination method v1.0 or EcoInvent 3.6 (2019). taking into account the sum of production energy and yarn twisting energy (which is
outsourced).
3.6 ALLOCATION For C1 the method and amount of the generic data set 'Polyester weefsel' from chapter
22.46 Grondwapening en grondscheiding of the DuboCalc programme (database version
NMD 1.8 - 5.01.14052018) was used. In this generic data set, 0.0013h work per m² of
Allocation is based on physical characteristics (mass). The production data was calculated geotextile was assumed.
according to the annual quantity by mass. The raw materials and energy were calculated
according to this allocation key.
3.9 DATA QUALITY
3.7 DATA COLLECTION & REFERENCE TIME PERIOD All process-specific data was collected for the 2021 operating year and is therefore up-to-
date. The data is based on the annual average. In order to ensure comparability of the
All process-specific data was collected for the operating year 2021. results, only consistent background data of the Ecoinvent database V3.6 was used in the
LCA (e.g., records on energy, transportation, and supplies), which refers to reference year
2019. The database is regularly reviewed and thus complies with the requirements of EN
3.8 ESTIMATES AND ASSUMPTIONS 15804 (background data not older than 10 years). All consistent datasets contained in the
Ecoinvent database are documented and can be viewed in the online Ecoinvent
Almost all the datasets selected for the LCA refer to the RoW as the geographical documentation. The primary data were provided by Gold-Joint. The life cycle was modelled
reference, as there were no specific environmental profiles available. with the R<THiNK EPD App.
Gold-Joint delivers its product to different countries, so the calculation of transport to
construction site (A4) was done by taking the average distance, weighted by the 3.10 GUARANTEES OF ORIGIN
proportion of product shipped to each country. For module A4, a data set for a non-
specific truck and a transoceanic ship was used. In this EPD, the local based approach was considered for the LCA, therefore no guaranties
The following inputs have been placed under cut-off criteria (<1% of the total mass): of origin (GO) are needed.
ACEGrid® | ReTHiNK-58054 8 / 25
Environmental Product Declaration
3 Calculation rules
3.12 SCALING
Parameter Value
Scaling type Linear
Description dimension mass for each geogrid
Dimension 0.000
Scalable dimension 1.000
Unit dimension kg/m²
ACEGrid® | ReTHiNK-58054 9 / 25
Environmental Product Declaration
4 Scenarios and additional technical information
4.1 TRANSPORT TO CONSTRUCTION SITE (A4)
For the transport from production place to assembly/user, the following scenario is
assumed for module A4 of this EPD.
Value and unit
Vehicle type used for transport Transoceanic ship / Lorry unspecified
Fuel type and consumption of vehicle
Distance 5383 km
Capacity utilisation (including empty returns)
Bulk density of transported products
Volume capacity utilisation factor
4.2 ASSEMBLY (A5)
The following information describes the scenarios for flows entering the system and flows
leaving the system at module A5.
FLOWS ENTERING THE SYSTEM
There are no significant environment impacts as a result of materials or energy used in the
construction stage (A5).
FLOWS LEAVING THE SYSTEM
The following output flows leaving the system at module A5 are assumed.
Description Value Unit
Output materials as result of loss during construction 5 %
Output materials as result of waste processing of materials used for installation/assembly at the building site 0.000 kg
Output materials as result of waste processing of used packaging 0.126 kg
4.3 DE-CONSTRUCTION, DEMOLITION (C1)
The following information describes the scenario for demolition at end of life.
Description Amount Unit
Hydraulic excavator (average) [NMD] 0.001 hr
ACEGrid® | ReTHiNK-58054 10 / 25
Environmental Product Declaration
4 Scenarios and additional technical information
4.4 TRANSPORT END-OF-LIFE (C2)
The following distances and transport conveyance are assumed for transportation during
end of life for the different types of waste processing.
Waste Scenario Transport conveyance Not removed (stays in Landfill Incineration Recycling Re-use
work) [km] [km] [km] [km] [km]
PE/PP soil reinforcement (geotextile and Lorry (Truck), unspecified (default) | market
0 100 150 50 0
geogrid 54) group for (GLO)
The transport conveyance(s) used in the scenario(s) for transport during end of life has the
following characteristics.
Value and unit
Vehicle type used for transport Lorry (Truck), unspecified (default) | market group for (GLO)
Fuel type and consumption of vehicle not available
Capacity utilisation (including empty returns) 50 % (loaded up and return empty)
Bulk density of transported products inapplicable
Volume capacity utilisation factor 1
4.5 END OF LIFE (C3, C4)
The scenario(s) assumed for end of life of the product are given in the following tables.
First the assumed percentages per type of waste processing are displayed, followed by the
assumed amounts.
Waste Scenario Region Not removed (stays in work) [%] Landfill [%] Incineration [%] Recycling [%] Re-use [%]
PE/PP soil reinforcement (geotextile and geogrid 54) NL 25 0 70 5 0
Waste Scenario Not removed (stays in work) [kg] Landfill [kg] Incineration [kg] Recycling [kg] Re-use [kg]
PE/PP soil reinforcement (geotextile and geogrid 54) 0.263 0.000 0.735 0.053 0.000
Total 0.263 0.000 0.735 0.053 0.000
ACEGrid® | ReTHiNK-58054 11 / 25
Environmental Product Declaration
4 Scenarios and additional technical information
4.6 BENEFITS AND LOADS BEYOND THE SYSTEM BOUNDARY (D)
The presented Benefits and loads beyond the system boundary in this EPD are based on
the following calculated Net output flows in kilograms and Energy recovery displayed in
MJ Lower Heating Value.
Waste Scenario Net output flow [kg] Energy recovery [MJ]
PE/PP soil reinforcement (geotextile and geogrid 54) 0.050 13.684
Total 0.050 13.684
ACEGrid® | ReTHiNK-58054 12 / 25
Environmental Product Declaration
5 Results
For the impact assessment, the characterization factors of the LCIA method EN 15804 +A2
Method v1.0 are used. Long-term emissions (>100 years) are not considered in the impact
assessment. The results of the impact assessment are only relative statements that do not
make any statements about end-points of the impact categories, exceedance of threshold
values, safety margins or risks. The following tables show the results of the indicators of the
impact assessment, of the use of resources as well as of waste and other output flows.
ACEGrid® | ReTHiNK-58054 13 / 25
Environmental Product Declaration
5 Results
5.1 ENVIRONMENTAL IMPACT INDICATORS PER SQUARE METER (FIXED PART)
CORE ENVIRONMENTAL IMPACT INDICATORS EN15804+A2
Abbreviation Unit A1 A2 A3 A4 A5 C1 C2 C3 C4 D
AP mol H+ eqv. 1.31E-3 -2.72E-5 4.66E-4 1.68E-4 1.34E-4 7.12E-4 2.15E-7 2.17E-6 5.92E-8 2.75E-6
GWP-total kg CO2 eqv. 2.07E-1 -4.58E-4 7.92E-2 1.43E-2 1.71E-1 6.81E-2 3.72E-5 4.81E-3 9.50E-5 1.39E-2
GWP-b kg CO2 eqv. 6.12E-4 4.92E-7 -1.59E-3 8.87E-6 1.48E-1 1.89E-5 1.71E-8 6.96E-7 7.31E-8 1.44E-6
GWP-f kg CO2 eqv. 2.06E-1 -4.58E-4 8.03E-2 1.43E-2 2.31E-2 6.81E-2 3.71E-5 4.81E-3 9.49E-5 1.40E-2
GWP-luluc kg CO2 eqv. 5.11E-4 -4.67E-7 5.15E-4 5.93E-6 5.38E-5 5.37E-6 1.36E-8 3.91E-7 3.35E-9 -3.60E-5
EP-m kg N eqv. 1.80E-4 -6.41E-6 1.26E-4 4.17E-5 3.11E-5 3.14E-4 7.59E-8 5.92E-7 3.59E-8 4.59E-7
EP-fw kg P eqv. 2.19E-4 8.91E-10 1.75E-5 1.69E-7 1.19E-5 2.48E-7 3.75E-10 1.45E-8 1.22E-10 -2.25E-7
EP-T mol N eqv. 2.00E-3 -7.13E-5 1.24E-3 4.65E-4 3.33E-4 3.45E-3 8.37E-7 6.60E-6 2.18E-7 6.60E-6
kg CFC 11
ODP 2.84E-8 -8.26E-11 7.03E-9 3.05E-9 3.00E-9 1.47E-8 8.20E-12 1.47E-10 2.10E-12 1.67E-9
eqv.
kg NMVOC
POCP 6.80E-4 -1.82E-5 2.97E-4 1.27E-4 1.01E-4 9.49E-4 2.39E-7 1.77E-6 8.33E-8 -3.25E-6
eqv.
ADP-f MJ 2.60E+0 -4.79E-3 1.13E+0 2.12E-1 2.63E-1 9.37E-1 5.60E-4 3.75E-3 1.61E-4 2.30E-1
ADP-mm kg Sb-eqv. 2.00E-6 4.86E-9 9.34E-7 2.50E-7 3.25E-7 1.04E-7 9.41E-10 6.17E-9 7.26E-11 -2.94E-8
m3 world
WDP 1.02E-1 7.76E-6 2.61E-2 9.29E-4 7.39E-3 1.26E-3 2.00E-6 2.45E-4 6.88E-6 4.78E-4
eqv.
AP=Acidification (AP) | GWP-total=Global warming potential (GWP-total) | GWP-b=Global warming potential - Biogenic (GWP-b) | GWP-f=Global warming potential - Fossil (GWP-f) | GWP-
luluc=Global warming potential - Land use and land use change (GWP-luluc) | EP-m=Eutrophication marine (EP-m) | EP-fw=Eutrophication, freshwater (EP-fw) | EP-T=Eutrophication,
terrestrial (EP-T) | ODP=Ozone depletion (ODP) | POCP=Photochemical ozone formation - human health (POCP) | ADP-f=Resource use, fossils (ADP-f) | ADP-mm=Resource use, minerals and
metals (ADP-mm) | WDP=Water use (WDP)
ACEGrid® | ReTHiNK-58054 14 / 25
Environmental Product Declaration
5 Results
ADDITIONAL ENVIRONMENTAL IMPACT INDICATORS EN15084+A2
Abbreviation Unit A1 A2 A3 A4 A5 C1 C2 C3 C4 D
ETP-fw CTUe 1.05E+1 -1.36E-3 7.98E+0 1.74E-1 1.11E+0 5.65E-1 4.99E-4 6.04E-2 1.71E-4 -8.09E-3
disease
PM 2.18E-8 1.33E-11 7.00E-9 1.01E-9 2.06E-9 1.89E-8 3.34E-12 1.76E-11 1.12E-12 -8.36E-11
incidence
HTP-c CTUh 9.45E-10 -3.19E-13 1.03E-10 5.72E-12 6.47E-11 1.97E-11 1.62E-14 9.20E-13 4.48E-15 -5.27E-13
HTP-nc CTUh 1.00E-7 7.48E-13 7.26E-9 1.77E-10 5.53E-9 4.85E-10 5.46E-13 1.91E-11 1.11E-13 -2.50E-11
IR kBq U235 eqv. 8.75E-3 -2.12E-5 2.62E-3 9.03E-4 9.06E-4 4.02E-3 2.35E-6 1.53E-5 6.29E-7 -2.65E-5
SQP Pt 5.42E-1 4.46E-3 2.83E+0 1.35E-1 2.05E-1 1.20E-1 4.86E-4 1.38E-3 3.80E-4 -4.52E+0
ETP-fw=Ecotoxicity, freshwater (ETP-fw) | PM=Particulate Matter (PM) | HTP-c=Human toxicity, cancer (HTP-c) | HTP-nc=Human toxicity, non-cancer (HTP-nc) | IR=Ionising radiation, human
health (IR) | SQP=Land use (SQP)
CLASSIFICATION OF DISCLAIMERS TO THE DECLARATION OF CORE AND ADDITIONAL ENVIRONMENTAL IMPACT INDICATORS
ILCD classification Indicator Disclaimer
Global warming potential (GWP) None
ILCD type / level 1 Depletion potential of the stratospheric ozone layer (ODP) None
Potential incidence of disease due to PM emissions (PM) None
AAcidification potential, Accumulated Exceedance (AP) None
Eutrophication potential, Fraction of nutrients reaching freshwater end compartment
None
(EP-freshwater)
Eutrophication potential, Fraction of nutrients reaching marine end compartment
ILCD type / level 2 None
(EP-marine)
Eutrophication potential, Accumulated Exceedance (EP-terrestrial) None
Formation potential of tropospheric ozone (POCP) None
Potential Human exposure efficiency relative to U235 (IRP) 1
Abiotic depletion potential for non-fossil resources (ADP-minerals&metals) 2
ILCD type / level 3
Abiotic depletion potential for fossil resources (ADP-fossil) 2
Water (user) deprivation potential, deprivation-weighted water consumption (WDP) 2
Potential Comparative Toxic Unit for ecosystems (ETP-fw) 2
ACEGrid® | ReTHiNK-58054 15 / 25
Environmental Product Declaration
5 Results
ILCD classification Indicator Disclaimer
Potential Comparative Toxic Unit for humans (HTP-c) 2
Potential Comparative Toxic Unit for humans (HTP-nc) 2
Potential Soil quality index (SQP) 2
Disclaimer 1 – This impact category deals mainly with the eventual impact of low dose ionizing radiation on human health of the nuclear fuel cycle. It does not consider effects due to possible
nuclear accidents, occupational exposure nor due to radioactive waste disposal in underground facilities. Potential ionizing radiation from the soil, from radon and from some construction
materials is also not measured by this indicator.
Disclaimer 2 – The results of this environmental impact indicator shall be used with care as the uncertainties on these results are high or as there is limited experienced with the indicator.
5.2 ENVIRONMENTAL IMPACT INDICATORS PER SQUARE METER (SCALABLE PART)
CORE ENVIRONMENTAL IMPACT INDICATORS EN15804+A2
Abbreviation Unit A1 A2 A3 A4 A5 C1 C2 C3 C4 D
AP mol H+ eqv. 1.17E-2 4.56E-4 1.50E-3 1.94E-3 8.76E-4 0.00E+0 8.40E-5 8.45E-4 2.31E-5 -9.45E-4
GWP-total kg CO2 eqv. 2.15E+0 1.60E-2 3.81E-1 1.66E-1 3.28E-1 0.00E+0 1.45E-2 1.87E+0 3.70E-2 -7.88E-1
GWP-b kg CO2 eqv. 4.55E-3 -2.97E-6 -1.03E-4 1.02E-4 2.64E-4 0.00E+0 6.68E-6 2.71E-4 2.85E-5 -7.44E-4
GWP-f kg CO2 eqv. 2.14E+0 1.60E-2 3.81E-1 1.65E-1 3.27E-1 0.00E+0 1.45E-2 1.87E+0 3.70E-2 -7.87E-1
GWP-luluc kg CO2 eqv. 3.15E-3 1.03E-5 2.33E-4 6.85E-5 1.89E-4 0.00E+0 5.30E-6 1.52E-4 1.31E-6 -5.28E-5
EP-m kg N eqv. 1.79E-3 1.13E-4 2.34E-4 4.82E-4 1.59E-4 0.00E+0 2.96E-5 2.31E-4 1.40E-5 -2.34E-4
EP-fw kg P eqv. 1.16E-3 8.05E-8 7.71E-5 1.95E-6 6.23E-5 0.00E+0 1.46E-7 5.65E-6 4.74E-8 -2.59E-6
EP-T mol N eqv. 1.97E-2 1.26E-3 2.59E-3 5.37E-3 1.75E-3 0.00E+0 3.26E-4 2.57E-3 8.49E-5 -2.57E-3
kg CFC 11
ODP 2.02E-7 3.27E-9 1.08E-8 3.52E-8 1.92E-8 0.00E+0 3.20E-9 5.73E-8 8.18E-10 -9.14E-8
eqv.
kg NMVOC
POCP 6.92E-3 3.28E-4 9.14E-4 1.47E-3 5.65E-4 0.00E+0 9.31E-5 6.91E-4 3.25E-5 -9.67E-4
eqv.
AP=Acidification (AP) | GWP-total=Global warming potential (GWP-total) | GWP-b=Global warming potential - Biogenic (GWP-b) | GWP-f=Global warming potential - Fossil (GWP-f) | GWP-
luluc=Global warming potential - Land use and land use change (GWP-luluc) | EP-m=Eutrophication marine (EP-m) | EP-fw=Eutrophication, freshwater (EP-fw) | EP-T=Eutrophication,
terrestrial (EP-T) | ODP=Ozone depletion (ODP) | POCP=Photochemical ozone formation - human health (POCP) | ADP-f=Resource use, fossils (ADP-f) | ADP-mm=Resource use, minerals and
metals (ADP-mm) | WDP=Water use (WDP)
ACEGrid® | ReTHiNK-58054 16 / 25
Environmental Product Declaration
5 Results
Abbreviation Unit A1 A2 A3 A4 A5 C1 C2 C3 C4 D
ADP-f MJ 3.73E+1 2.11E-1 5.69E+0 2.45E+0 2.50E+0 0.00E+0 2.18E-1 1.46E+0 6.26E-2 -1.52E+1
ADP-mm kg Sb-eqv. 2.85E-5 1.63E-7 2.60E-6 2.89E-6 2.00E-6 0.00E+0 3.67E-7 2.40E-6 2.83E-8 -1.16E-6
m3 world
WDP 1.02E+0 3.86E-4 9.23E-2 1.07E-2 6.71E-2 0.00E+0 7.81E-4 9.56E-2 2.68E-3 -1.37E-1
eqv.
AP=Acidification (AP) | GWP-total=Global warming potential (GWP-total) | GWP-b=Global warming potential - Biogenic (GWP-b) | GWP-f=Global warming potential - Fossil (GWP-f) | GWP-
luluc=Global warming potential - Land use and land use change (GWP-luluc) | EP-m=Eutrophication marine (EP-m) | EP-fw=Eutrophication, freshwater (EP-fw) | EP-T=Eutrophication,
terrestrial (EP-T) | ODP=Ozone depletion (ODP) | POCP=Photochemical ozone formation - human health (POCP) | ADP-f=Resource use, fossils (ADP-f) | ADP-mm=Resource use, minerals and
metals (ADP-mm) | WDP=Water use (WDP)
ADDITIONAL ENVIRONMENTAL IMPACT INDICATORS EN15084+A2
Abbreviation Unit A1 A2 A3 A4 A5 C1 C2 C3 C4 D
ETP-fw CTUe 7.16E+1 1.45E-1 7.91E+0 2.02E+0 6.46E+0 0.00E+0 1.95E-1 2.36E+1 6.66E-2 -1.27E+0
disease
PM 1.61E-7 6.39E-10 1.42E-8 1.17E-8 1.02E-8 0.00E+0 1.30E-9 6.85E-9 4.35E-10 -4.80E-9
incidence
HTP-c CTUh 5.74E-9 8.76E-12 4.12E-10 6.60E-11 3.48E-10 0.00E+0 6.32E-12 3.59E-10 1.75E-12 -7.15E-11
HTP-nc CTUh 5.31E-7 1.25E-10 3.48E-8 2.04E-9 2.92E-8 0.00E+0 2.13E-10 7.45E-9 4.33E-11 -1.28E-9
IR kBq U235 eqv. 6.91E-2 9.00E-4 8.65E-3 1.04E-2 5.20E-3 0.00E+0 9.15E-4 5.98E-3 2.45E-4 -6.22E-3
SQP Pt 5.32E+0 5.56E-2 5.80E-1 1.56E+0 4.59E-1 0.00E+0 1.89E-1 5.38E-1 1.48E-1 -2.90E-1
ETP-fw=Ecotoxicity, freshwater (ETP-fw) | PM=Particulate Matter (PM) | HTP-c=Human toxicity, cancer (HTP-c) | HTP-nc=Human toxicity, non-cancer (HTP-nc) | IR=Ionising radiation, human
health (IR) | SQP=Land use (SQP)
CLASSIFICATION OF DISCLAIMERS TO THE DECLARATION OF CORE AND ADDITIONAL ENVIRONMENTAL IMPACT INDICATORS
ILCD classification Indicator Disclaimer
Global warming potential (GWP) None
ILCD type / level 1 Depletion potential of the stratospheric ozone layer (ODP) None
Potential incidence of disease due to PM emissions (PM) None
AAcidification potential, Accumulated Exceedance (AP) None
ILCD type / level 2
None
ACEGrid® | ReTHiNK-58054 17 / 25
Environmental Product Declaration
5 Results
ILCD classification Indicator Disclaimer
Eutrophication potential, Fraction of nutrients reaching freshwater end compartment
(EP-freshwater)
Eutrophication potential, Fraction of nutrients reaching marine end compartment
None
(EP-marine)
Eutrophication potential, Accumulated Exceedance (EP-terrestrial) None
Formation potential of tropospheric ozone (POCP) None
Potential Human exposure efficiency relative to U235 (IRP) 1
Abiotic depletion potential for non-fossil resources (ADP-minerals&metals) 2
Abiotic depletion potential for fossil resources (ADP-fossil) 2
Water (user) deprivation potential, deprivation-weighted water consumption (WDP) 2
ILCD type / level 3 Potential Comparative Toxic Unit for ecosystems (ETP-fw) 2
Potential Comparative Toxic Unit for humans (HTP-c) 2
Potential Comparative Toxic Unit for humans (HTP-nc) 2
Potential Soil quality index (SQP) 2
Disclaimer 1 – This impact category deals mainly with the eventual impact of low dose ionizing radiation on human health of the nuclear fuel cycle. It does not consider effects due to possible
nuclear accidents, occupational exposure nor due to radioactive waste disposal in underground facilities. Potential ionizing radiation from the soil, from radon and from some construction
materials is also not measured by this indicator.
Disclaimer 2 – The results of this environmental impact indicator shall be used with care as the uncertainties on these results are high or as there is limited experienced with the indicator.
ACEGrid® | ReTHiNK-58054 18 / 25
Environmental Product Declaration
5 Results
5.3 ENVIRONMENTAL IMPACT INDICATORS PER SQUARE METER (FIXED PART)
PARAMETERS DESCRIBING RESOURCE USE
Abbreviation Unit A1 A2 A3 A4 A5 C1 C2 C3 C4 D
PERE MJ 2.17E-1 8.03E-6 5.47E-1 3.16E-3 4.09E-2 5.07E-3 7.01E-6 3.79E-4 2.84E-6 -7.79E-1
PERM MJ 0.00E+0 0.00E+0 0.00E+0 0.00E+0 0.00E+0 0.00E+0 0.00E+0 0.00E+0 0.00E+0 0.00E+0
PERT MJ 2.17E-1 8.03E-6 5.47E-1 3.16E-3 4.09E-2 5.07E-3 7.01E-6 3.79E-4 2.84E-6 -7.79E-1
PENRE MJ 3.32E+0 -5.08E-3 2.42E-2 2.25E-1 2.47E-1 9.95E-1 5.95E-4 3.98E-3 1.71E-4 2.65E-1
PENRM MJ -5.67E-1 0.00E+0 1.20E+0 0.00E+0 3.27E-2 0.00E+0 0.00E+0 0.00E+0 0.00E+0 -8.39E-3
PENRT MJ 2.75E+0 -5.08E-3 1.22E+0 2.25E-1 2.80E-1 9.95E-1 5.95E-4 3.98E-3 1.71E-4 2.56E-1
SM Kg 0.00E+0 0.00E+0 0.00E+0 0.00E+0 0.00E+0 0.00E+0 0.00E+0 0.00E+0 0.00E+0 0.00E+0
RSF MJ 0.00E+0 0.00E+0 0.00E+0 0.00E+0 0.00E+0 0.00E+0 0.00E+0 0.00E+0 0.00E+0 0.00E+0
NRSF MJ 0.00E+0 0.00E+0 0.00E+0 0.00E+0 0.00E+0 0.00E+0 0.00E+0 0.00E+0 0.00E+0 0.00E+0
FW M3 2.82E-3 2.37E-7 8.99E-4 3.04E-5 2.23E-4 4.83E-5 6.82E-8 7.21E-6 1.68E-7 2.77E-6
PERE=renewable primary energy ex. raw materials | PERM=renewable primary energy used as raw materials | PERT=renewable primary energy total | PENRE=non-renewable primary energy
ex. raw materials | PENRM=non-renewable primary energy used as raw materials | PENRT=non-renewable primary energy total | SM=use of secondary material | RSF=use of renewable
secondary fuels | NRSF=use of non-renewable secondary fuels | FW=use of net fresh water
OTHER ENVIRONMENTAL INFORMATION DESCRIBING WASTE CATEGORIES
Abbreviation Unit A1 A2 A3 A4 A5 C1 C2 C3 C4 D
HWD Kg 2.13E-7 6.92E-9 1.17E-6 4.20E-7 2.69E-7 2.55E-6 1.42E-9 7.14E-9 2.44E-10 2.42E-7
NHWD Kg 2.09E-2 4.15E-4 1.54E-2 9.20E-3 4.66E-3 1.11E-3 3.55E-5 9.24E-5 6.42E-4 -6.43E-4
RWD Kg 6.07E-6 -3.60E-8 2.62E-6 1.39E-6 9.07E-7 6.51E-6 3.68E-9 1.35E-8 9.55E-10 -3.41E-8
HWD=hazardous waste disposed | NHWD=non hazardous waste disposed | RWD=radioactive waste disposed
ACEGrid® | ReTHiNK-58054 19 / 25
Environmental Product Declaration
5 Results
ENVIRONMENTAL INFORMATION DESCRIBING OUTPUT FLOWS
Abbreviation Unit A1 A2 A3 A4 A5 C1 C2 C3 C4 D
CRU Kg 0.00E+0 0.00E+0 0.00E+0 0.00E+0 0.00E+0 0.00E+0 0.00E+0 0.00E+0 0.00E+0 0.00E+0
MFR Kg 0.00E+0 0.00E+0 2.45E-3 0.00E+0 6.81E-2 0.00E+0 0.00E+0 1.28E-4 0.00E+0 0.00E+0
MER Kg 0.00E+0 0.00E+0 0.00E+0 0.00E+0 0.00E+0 0.00E+0 0.00E+0 0.00E+0 0.00E+0 0.00E+0
EET MJ 0.00E+0 0.00E+0 -1.56E-2 0.00E+0 0.00E+0 0.00E+0 0.00E+0 0.00E+0 0.00E+0 -1.19E-1
EEE MJ 0.00E+0 0.00E+0 -9.03E-3 0.00E+0 0.00E+0 0.00E+0 0.00E+0 0.00E+0 0.00E+0 -6.90E-2
CRU=Components for re-use | MFR=Materials for recycling | MER=Materials for energy recovery | EET=Exported Energy Thermic | EEE=Exported Energy Electric
5.4 ENVIRONMENTAL IMPACT INDICATORS PER SQUARE METER (SCALABLE PART)
PARAMETERS DESCRIBING RESOURCE USE
Abbreviation Unit A1 A2 A3 A4 A5 C1 C2 C3 C4 D
PERE MJ 1.73E+0 1.63E-3 1.90E-1 3.65E-2 1.14E-1 0.00E+0 2.73E-3 1.48E-1 1.11E-3 -8.88E-2
PERM MJ 0.00E+0 0.00E+0 0.00E+0 0.00E+0 0.00E+0 0.00E+0 0.00E+0 0.00E+0 0.00E+0 0.00E+0
PERT MJ 1.73E+0 1.63E-3 1.90E-1 3.65E-2 1.14E-1 0.00E+0 2.73E-3 1.48E-1 1.11E-3 -8.88E-2
PENRE MJ 1.98E+1 2.24E-1 3.30E+0 2.60E+0 1.52E+0 0.00E+0 2.32E-1 1.55E+0 6.66E-2 -1.44E+1
PENRM MJ 2.01E+1 0.00E+0 2.75E+0 0.00E+0 1.15E+0 0.00E+0 0.00E+0 0.00E+0 0.00E+0 -2.29E+0
PENRT MJ 3.99E+1 2.24E-1 6.05E+0 2.60E+0 2.67E+0 0.00E+0 2.32E-1 1.55E+0 6.66E-2 -1.67E+1
SM Kg 0.00E+0 0.00E+0 0.00E+0 0.00E+0 0.00E+0 0.00E+0 0.00E+0 0.00E+0 0.00E+0 0.00E+0
RSF MJ 0.00E+0 0.00E+0 0.00E+0 0.00E+0 0.00E+0 0.00E+0 0.00E+0 0.00E+0 0.00E+0 0.00E+0
NRSF MJ 0.00E+0 0.00E+0 0.00E+0 0.00E+0 0.00E+0 0.00E+0 0.00E+0 0.00E+0 0.00E+0 0.00E+0
FW M3 2.71E-2 1.36E-5 2.83E-3 3.52E-4 1.81E-3 0.00E+0 2.66E-5 2.81E-3 6.53E-5 -1.97E-3
PERE=renewable primary energy ex. raw materials | PERM=renewable primary energy used as raw materials | PERT=renewable primary energy total | PENRE=non-renewable primary energy
ex. raw materials | PENRM=non-renewable primary energy used as raw materials | PENRT=non-renewable primary energy total | SM=use of secondary material | RSF=use of renewable
secondary fuels | NRSF=use of non-renewable secondary fuels | FW=use of net fresh water
ACEGrid® | ReTHiNK-58054 20 / 25
Environmental Product Declaration
5 Results
OTHER ENVIRONMENTAL INFORMATION DESCRIBING WASTE CATEGORIES
Abbreviation Unit A1 A2 A3 A4 A5 C1 C2 C3 C4 D
HWD Kg 4.07E-5 2.53E-7 2.64E-6 4.85E-6 2.81E-6 0.00E+0 5.53E-7 2.78E-6 9.52E-8 -1.48E-5
NHWD Kg 2.08E-1 2.76E-3 3.56E-2 1.06E-1 3.92E-2 0.00E+0 1.39E-2 3.60E-2 2.50E-1 -8.04E-3
RWD Kg 5.60E-5 1.45E-6 7.29E-6 1.60E-5 4.77E-6 0.00E+0 1.43E-6 5.25E-6 3.72E-7 -7.72E-6
HWD=hazardous waste disposed | NHWD=non hazardous waste disposed | RWD=radioactive waste disposed
ENVIRONMENTAL INFORMATION DESCRIBING OUTPUT FLOWS
Abbreviation Unit A1 A2 A3 A4 A5 C1 C2 C3 C4 D
CRU Kg 0.00E+0 0.00E+0 0.00E+0 0.00E+0 0.00E+0 0.00E+0 0.00E+0 0.00E+0 0.00E+0 0.00E+0
MFR Kg 0.00E+0 0.00E+0 1.32E-2 0.00E+0 5.17E-3 0.00E+0 0.00E+0 4.99E-2 0.00E+0 0.00E+0
MER Kg 0.00E+0 0.00E+0 0.00E+0 0.00E+0 0.00E+0 0.00E+0 0.00E+0 0.00E+0 0.00E+0 0.00E+0
EET MJ 0.00E+0 0.00E+0 2.75E-1 0.00E+0 0.00E+0 0.00E+0 0.00E+0 0.00E+0 0.00E+0 5.05E+0
EEE MJ 0.00E+0 0.00E+0 1.60E-1 0.00E+0 0.00E+0 0.00E+0 0.00E+0 0.00E+0 0.00E+0 2.93E+0
CRU=Components for re-use | MFR=Materials for recycling | MER=Materials for energy recovery | EET=Exported Energy Thermic | EEE=Exported Energy Electric
ACEGrid® | ReTHiNK-58054 21 / 25
Environmental Product Declaration
5 Results
5.5 INFORMATION ON BIOGENIC CARBON CONTENT PER SQUARE METER
BIOGENIC CARBON CONTENT
The following Information describes the biogenic carbon content in (the main parts of) the
product at the factory gate per square meter:
Biogenic carbon content Amount Unit
Biogenic carbon content in the product 0 kg C
Biogenic carbon content in accompanying packaging 0 kg C
ACEGrid® | ReTHiNK-58054 22 / 25
Environmental Product Declaration
6 Interpretation of results
As shown in the figure below, raw material supply (A1) dominates in most environmental
core indicators. In some environmental core indicators waste processing (C3) and
production process (A3) have a great impact. The highest influence on the Global
Warming Potential (GWP-total) has raw material supply (A1), followed by waste processing
(C3).
ACEGrid® | ReTHiNK-58054 23 / 25
Environmental Product Declaration
7 References
ISO 14040
ISO 14040:2006-10, Environmental management - Life cycle assessment - Principles and
framework; EN ISO 14040:2006
ISO 14044
ISO 14044:2006-10, Environmental management - Life cycle assessment - Requirements
and guidelines; EN ISO 14040:2006
ISO 14025
ISO 14025:2011-10: Environmental labels and declarations — Type III environmental
declarations — Principles and procedures
EN 15804+A2
EN 15804+A2: 2019: Sustainability of construction works — Environmental Product
Declarations — Core rules for the product category of construction products
PCR A: General Program Category Rules for Construction Products from the EPD program
Kiwa-Ecobility Experts, 2022-02-14
PCR B: Product Category Rules (PCR) from the Kiwa-Ecobility Experts (Kiwa-EE) – Specific
Product Category Rules: Geosynthetic products, 2023-07-21
ACEGrid® | ReTHiNK-58054 24 / 25
Environmental Product Declaration
8 Contact information
Publisher Operator Owner of declaration
Kiwa-Ecobility Experts Kiwa-Ecobility Experts Gold-Joint Industry Co., Ltd.
Voltastraße 5 Voltastraße 5 No.33, Jing 3 Rd. Wuqi Dist.
13355 Berlin, DE 13355 Berlin, DE 43541 Taichung City, Taiwan (R.O.C.), TW
E-mail: E-mail: E-mail:
DE.Ecobility.Experts@kiwa.com DE.Ecobility.Experts@kiwa.com marketing@geoace.com
Website: Website: Website:
https://www.kiwa.com/de/en/themes/ecobility-experts/ecobility-https://www.kiwa.com/de/en/themes/ecobility-experts/ecobility-www.geoace.com
experts-epd-program/ experts-epd-program/
Kiwa-Ecobility Experts is
established member of the
ACEGrid® | ReTHiNK-58054 25 / 25
