ENVIRONMENTAL PRODUCT DECLARATION
as per ISO 14025 and EN 15804+A2
Owner of the Declaration Etex Building Performance International
Programme holder Institut Bauen und Umwelt e.V. (IBU)
Publisher Institut Bauen und Umwelt e.V. (IBU)
Declaration number EPD-PMT-20210155-IBC2-EN
Issue date 30.11.2021
Valid to 05.09.2026
PROMATECT®-100 / PROMATECT®-200 /
PROMATECT®-250 / PROMAXON®-Typ A
Mineral bound light weight fire protective boards
Promat
www.ibu-epd.com | https://epd-online.com
Umwelt Produktdeklaration Name des Herstellers – Name des Produkts
1. General Information
Etex Building Performance NV PROMATECT®-100/
PROMATECT®-200/
PROMATECT®-250/
PROMAXON®-Typ A
Programme holder Owner of the declaration
IBU – Institut Bauen und Umwelt e.V. Etex Building Performance International
Panoramastr. 1 500 Rue Marcel Demonque
10178 Berlin F-84915 Avignon
Germany France
Declaration number Declared product / declared unit
EPD-PMT-20210155-IBC2-EN The functional unit is 1 m² of PROMATECT®-
100/200/250 and PROMAXON®-TYP A with a
thickness of 15 mm.
This declaration is based on the product Scope:
category rules: The life cycle assessment is based on production data
Calcium silicate insulating materials, 11.2017 of PROMATECT®-100, PROMATECT®-
(PCR checked and approved by the SVR) 200, PROMATECT®-250 and PROMAXON®- Typ A of
the year 2019 at the production site Tisselt, Belgium.
Issue date
30.11.2021
The owner of the declaration shall be liable for the
Valid to underlying information and evidence; the IBU shall not
be liable with respect to manufacturer information, life
05.09.2026
cycle assessment data and evidences.
The EPD was created according to the specifications
of EN 15804+A2. In the following, the standard will be
simplified as EN 15804.
Verification
The standard EN 15804 serves as the core PCR
Independent verification of the declaration and data
according to ISO 14025:2010
Dipl. Ing. Hans Peters internally x externally
(chairman of Institut Bauen und Umwelt e.V.)
Dr. Alexander Röder Vito D'Incognito
(Managing Director Institut Bauen und Umwelt e.V.)) (Independent verifier)
2. Product
2.1 Product description/Product definition  ETA 07/0297_2018-03-25_PROMATECT®-
PROMATECT®-100/200/250 and PROMAXON®-Typ 200;
A are fire protective calcium silicate boards, mineral
 ETA 08/0161_2018-03-25_PROMATECT®-
bound with mineral fillers.
250;
All boards are manufactured in the same plant, using
the same production technology and similar raw  ETA 06/0215_2015-09-18_PROMAXON®-
materials though in different quantities. Typ A
The functional unit refers to a weighted average
product based on the ratio of tons produced of all
and the CE-marking. For the application and use the
products in the reference year 2019.
respective national provisions apply.
For the placing of the product on the market in the
2.2 Application
European Union/European Free Trade Association
All boards are used in interior building applications
/EU/EFTA) (with the exception of Switzerland) the
where normal to high levels of fire resistance are
Regulation (EU) No. 305/2011 (CPR) applies. The
required.
products need a declaration of performance taking into
The boards are intended for the manufacture or
consideration
cladding of building components, for
 ETA 06/0219_2018-06-25_PROMATECT®-
filling aluminium/steel profiles and for fire protection of
100; ducts.
2 Environmental Product Declaration Etex Building Performance NV – PROMATECT®-100 / PROMATECT®-200 /
PROMATECT®-250 / PROMAXON® Typ A
slurry. The slurry is formed to a board. Boards are
2.3 Technical Data dried and edges are trimmed. All material which is cut
off is fully recycled within the production plant.
Constructional data
Name Value Unit
Gross density 23°C, 50% RH;
according to ETA 06/0219, ETA 680 -
kg/m3
06/0215, ETA 07/0297 and ETA 970
08/0161
Compressive strength according to EN
6.6 N/mm2
826
Tensile strength (perpendicular)
0.043 N/mm2
according to EN 1607
Flexural strength according to EN
>3 N/mm2
12467
Thermal conductivity according to EN
0.27 W/(mK)
12667 The quality management system of the company and
Water vapour diffusion resistance 3 - the production facility are certified according to ISO
factor according to EN 12572 9001.
Tensile strength (parallel) according to
1.21 N/mm^2
EN 1608
Values are guidance values and do not reflect a 2.7 Environment and health during
statistical evaluation or guaranteed value. manufacturing
Promat commits to a clean, healthy and safe working
Performance data of the product in accordance with environment for every person working in and for the
the declaration of performance with respect to its company.
essential characteristics according to ETA 06/0219; The company and the manufacturing site have an
ETA 07/0297; ETA 08/0161 and ETA 06/0215. environment, health and safety management system
which is ISO 14001 and ISO 45001 certified. The
manufacturing plant adheres to the Belgium
environmental and health and safety regulations.
2.4 Delivery status
Fire protective calcium silicate boards are 1200 x 2500
mm and are delivered in various thicknesses : 2.8 Product processing/Installation
 PROMATECT®-100 and PROMAXON®- Typ The fire protective board is cut and machined using
A : 8,10,12,15,18,20,25 mm conventional woodworking equipment.
 PROMATECT®-200 and PROMATECT®-250: Fixing the boards will require appropriate means,
which will depend upon the application and bearing
12,15,18,20,25,30 mm
structure. Boards can be installed using screws or
glues.
Industrial and environmental protection are assured
2.5 Base materials/Ancillary materials through training and coaching staff on safety and
Main raw materials used (in weight percentages): environmental impacts. Dust levels are kept low by
- sand: 5-20% performing dust extraction. Noise is reduced by noise
- lime: 2-15% insulation on the machines and ear protection is
- calcium silicate: 2-15% provided for persons entering the production area.
- gypsum: >50% Regular measurements on noise and dust are
- fibres: <3% performed and show conformity to the permitted
Reaction is performed in an aqueous suspension. levels.
All national, local and other applicable safety
This article contains substances listed in the candidate regulations are complied with.
list (date: 19.01.2021) exceeding 0.1 percentage by
mass: no. 2.9 Packaging
This article contains other carcinogenic, mutagenic, All fire protection boards are packed onto wooden
reprotoxic (CMR) substances in categories 1A or 1B pallets, wrapped with steel strapping tape and
which are not on the candidate list, exceeding 0.1 strengthened with cardboard corners.
percentage by mass: no.
Biocide products were added to this construction
product or it has been treated with biocide products 2.10 Condition of use
(this then concerns a treated product as defined by the After installation, the boards are resistant to the effects
(EU) Ordinance on Biocide Products No. 528/2012): of moisture and will not physically deteriorate when
no. used in damp or humid conditions. Performance
characteristics are not degraded by age or moisture.
Boards do not encourage mould growth and are
2.6 Manufacture resistant to attacks by insects or vermin.
The raw materials are mixed in water and blended in a
reactor to form calcium silicate. This is combined in a
mixer with the other raw materials to form a thick
3 Environmental Product Declaration Etex Building Performance NV – PROMATECT®-100 / PROMATECT®-200 /
PROMATECT®-250 / PROMAXON® Typ A
2.11 Environment and health during use damage of the components needs to be repaired using
When the product is used as designed, the current materials specified by the ETA of the specific products.
state of knowledge indicates that there is no risk Besides the need for repair, the destruction will not
involved for the environment or health. have any significant environmental impact.
2.12 Reference service life 2.14 Re-use phase
The service life according to the "Bundesinstitut für Several possibilities exist for the boards after the end-
Bau-, Stadt- und Raumforschung" (BBSR) table is of-life of the application in which they were used.
indicated to be ≥ 50 years. If the boards are removed non-destructively by
The reference service life (RSL) is therefore estimated releasing the screws, the undamaged product can be
to be 50 years. This RSL corresponds to the period re-used in accordance with the original purpose.
after which a building renovation is usually needed, If not contaminated with other building construction
independently of the actual lifetime of the product material, the boards also allow being recycled by the
(which can be longer than 50 years). manufacturer.
Furthermore, the products referred to could be used as
filler and bulk material in civil engineering.
For this EPD, a conservative worst-case scenario was
2.13 Extraordinary effects chosen at the end of life stage and the product was
sent for 100% to landfill.
Fire
The boards have a reaction to fire classification A1 or 2.15 Disposal
non-combustible according to EN13501-1. Within the production process, generated waste is re-
used within the process.
Fire protection When after end-of-life re-using or recycling the boards
Name Value as described in the previous paragraph is not practical,
Building material class A1 the boards can be disposed to landfill without pre-
Burning droplets - treatment thanks to the largely mineral ingredients
Smoke gas development - resulting in an inert matrix, The waste code in
accordance with the European List of Waste is
Water 170904.
The boards will not break when exposed to excessive
amounts of water, e.g. in case of flooding. Since the
raw materials used are of mineral origin, environmental 2.16 Further information
or health risks are avoided. However, the biological Further information is available on the following web
and chemical oxygen demand could increase if some site :
biodegradable components are dissolved in the water. https://www.promat.com
Mechanical destruction
In order to prevent any reduction of fire performance
following unforeseeable mechanical destruction, all
3. LCA: Calculation rules
3.1 Declared Unit (multiply results by this factor to
The declared unit is 1 m² of PROMATECT®- obtain the results for 1m² 10 mm)
100/200/250 and PROMAXON®-Typ A with a Adjustment factor to 1m² 12 mm
thickness of 15 mm. (multiply results by this factor to 0.80 -
The results for other thicknesses can be obtained by obtain the results for 1m² 12 mm)
multiplying the presented results by the corresponding Adjustment factor to 1m² 18 mm
adjustment factor as included in the table. (multiply results by this factor to 1.20 -
The unit refers to a weighted average product based obtain the results for 1m² 18 mm)
on the ratio of tons produced of all products in the Adjustment factor to 1m² 20 mm
reference year 2019. (multiply results by this factor to 1.33 -
obtain the results for 1m² 20 mm)
Declared unit Adjustment factor to 1m² 25 mm
Name Value Unit (multiply results by this factor to 1.67 -
Gross density 854 kg/m3 obtain the results for 1m² 25 mm)
Grammage 12.8 kg/m2 Adjustment factor to 1m² 30 mm
Declared unit 1.00 m² (multiply results by this factor to 2.00 -
Conversion factor to 1 kg (divide obtain the results for 1m² 30 mm))
results by this factor to obtain the 12.8 -
results for 1 kg) All boards declared in this EPD are produced at the
Adjustment factor to 1 ton Etex Building Performance production site in Tisselt
(multiply results by this factor to 78.13 - using the same production technology and similar raw
obtain the results for 1 ton) materials though in different quantities. The calculation
Adjustment factor to 1m² 8 mm of the weighted average recipe and grammage is
(multiply results by this factor to 0.53 - based on the ratio of tons produced of
obtain the results for 1m² 8 mm) PROMATECT®-100/-200/-250 and PROMAXON®-Typ
Adjustment factor to 1m² 10 mm 0.67 - A in 2019.
4 Environmental Product Declaration Etex Building Performance NV – PROMATECT®-100 / PROMATECT®-200 /
PROMATECT®-250 / PROMAXON® Typ A
treatment, which will result in an overestimation of
impacts.
3.2 System boundary All assumptions and approximations were documented
Type of the EPD: cradle to grave. precisely.
The following life cycle stages and modules are
included: 3.4 Cut-off criteria
In the assessment, all utilised raw material, thermal
Production stage (A1-A3): energy and electric power were considered
 pre-chains of the raw materials and their using GaBi datasets. Only the transport of packaging,
transportation to the manufacturing site production waste to recycling/disposal and of
installation loss waste to recycling was cut-off in this
 energy consumption during production
study and one polymeric additive having no
 recycling and disposal of production wastes
environmental relevance and used at less than 0.1%.
 production of packaging Production of capital equipment, facilities and
infrastructure required for the manufacture are outside
the scope of the study and thus were not included.
Construction stage (A4-A5):
3.5 Background data
 transportation of product to the construction
Background data were sourced from GaBi 10 database
site
version 2021.
 disposal of installation wastes
 incineration of packaging materials (potential 3.6 Data quality
benefits from energy substitution within the This study is mainly based on primary data collected
incineration process are declared in module directly from the manufacturing site and therefore data
quality can be assumed to be very good.
D)
The last update of the GaBi database used for
the background data was February 2021.
Use stage (B1-B7): 3.7 Period under review
 efforts for the use of the product, Data for the entire production period of 2019 were
maintenance and operational efforts collected and used for this EPD.
 modules B3, B4, B5 are declared as MNR
3.8 Allocation
(module not relevant) according to the IBU
Allocation in background data
requirement. These modules are defined on
Specific information on allocation within the
building level in general background data is given in the GaBi documentation.
Allocation in foreground data
The production process does not deliver any co-
End-of-life stage (C1-C4): products. In modules A1 to A3, specific raw material
and transport data were available, energy, waste and
 transport to disposal of the material
water could not be directly allocated to the product and
 landfill end-of-life scenario was considered
were allocated via the production volume of the
specific products.
Allocation for waste materials
Loads and benefits beyond system boundary (D): The environmental burden of the incineration of
 loads and benefits from recycling of packaging in the construction process stage is
production waste and incineration of assigned to the system (A5); resulting credits for
thermal and electrical energy are declared in module
packaging waste
D.
3.3 Estimates and assumptions 3.9 Comparability
Most of the input and output influences of the Life Basically, a comparison or an evaluation of EPD data
Cycle Inventory Analysis could be depicted using is only possible if all the data sets to be compared
corresponding data from the GaBi database. were created according to EN 15804 and the building
Assumptions and approximations were applied in case context, respectively the product-specific
of a lack of representative data. characteristics of performance, are taken into account.
There were no data records in the GaBi database
available for the wooden pallets, they were GaBi database version 2021.1 serves as background
approximated using the "Solid construction timber" database for the calculation of the life cycle
dataset. assessment.
The waste water treatment of process water was
approximated by datasets of municipal waste water
4. LCA: Scenarios and additional technical information
Characteristic product properties biogenic carbon in the construction product leaving the
Information on biogenic Carbon factory gate. It is declared separately for the product
The biogenic carbon content quantifies the amount of and for the accompanying packaging.
5 Environmental Product Declaration Etex Building Performance NV – PROMATECT®-100 / PROMATECT®-200 /
PROMATECT®-250 / PROMAXON® Typ A
Information on describing the biogenic Carbon Litres of fuel - l/100km
Content at factory gate Replacement of worn parts - kg
Name Value Unit
Biogenic Carbon Content in product 0.014 kg C
Biogenic Carbon Content in Reference service life
0.27 kg C
accompanying packaging Name Value Unit
Reference service life - a
Life Span (according to BBSR) >=50 a
Life Span according to the
- a
manufacturer
Transport to the building site (A4) Declared product properties (at the
- -
For the transport from the factory gate to the building gate) and finishes
site, an average distance of 100km was assumed. This Design application parameters (if
distance can be assumed to be representative of instructed by the manufacturer),
deliveries within Belgium. including the references to the - -
Name Value Unit appropriate practices and application
Litres of fuel 0.027 l/100km codes
Transport distance 100 km An assumed quality of work, when
Capacity utilisation (including empty installed in accordance with the - -
61 %
runs) manufacturer’s instructions
Gross density of products transported 854 kg/m3 Outdoor environment, (for outdoor
applications), e.g. weathering,
pollutants, UV and wind exposure, - -
Installation into the building (A5) building orientation, shading,
Only waste treatment of installation loss and packaging temperature
is considered in this module. Indoor environment (for indoor
Installation into the building (A5) applications), e.g. temperature, - -
Name Value Unit moisture, chemical exposure
Material loss 0.64 kg Usage conditions, e.g. frequency of
VOC in the air 0 kg use, mechanical exposure - -
Maintenance e.g. required frequency,
type and quality and replacement of - -
Use or application of the installed product (B1) see components
section 2.12 "Use"
No efforts and releases of substances occur during the Operational energy use (B6) and Operational water
normal (i.e. anticipated) use phase. use (B7)
No efforts occur in modules B6 and B7.
Name Value Unit Name Value Unit
Water consumption 0 m3
Maintenance (B2) Electricity consumption 0 kWh
No efforts occur during maintenance. Other energy carriers 0 MJ
Name Value Unit Equipment output 0 kW
Number/
Maintenance cycle 0
RSL End-of-life (C1-C4)
Water consumption 0 m3 A conservative approach was used in this study.
Auxiliary 0 kg Although after end-of-life, scenarios where the
Other resources 0 kg boards are re-used or recycled are realistic, a
Electricity consumption 0 kWh scenario with 100% landfill was used.
Other energy carriers 0 MJ Name Value Unit
Material loss 0 kg Landfilling 12.8 kg
Repair (B3) Reuse, recovery and/or recycling potentials (D),
Name Value Unit relevant scenario information
Information on the repair process - - Although re-use and recycling of the boards at the end
Information on the inspection process - - of life is possible, this is not yet a widely established
Number/ practice. Therefore, no possible benefits of recycling or
Repair cycle - RSL re-use of the boards were taken into account in this
Water consumption - m3 study. In module D, only the benefits from recycling of
production waste and incineration of waste packaging
Auxiliary - kg
were taken into account.
Other resources - kg
Name Value Unit
Electricity consumption - kWh
Exported electrical energy 1.65 MJ
Other energy carriers - MJ
Exported thermal energy 2.97 MJ
Material loss - kg
Replacement (B4) / Refurbishment (B5)
Name Value Unit
Number/
Replacement cycle -
RSL
Electricity consumption - kWh
6 Environmental Product Declaration Etex Building Performance NV – PROMATECT®-100 / PROMATECT®-200 /
PROMATECT®-250 / PROMAXON® Typ A
5. LCA: Results
The following tables depict the results of the indicators for the Life Cycle Assessment, use of resources and waste
with reference to 1 m² of PROMATECT®-100, PROMATECT®-200, PROMATECT®-250 and PROMAXON®-Typ
A with a thickness of 15 mm.
Disclaimer:
EP-freshwater: This indicator has been calculated as “kg P eq” as required in the characterization
model (EUTREND model, Struijs et al., 2009b, as implemented in ReCiPe;
http://eplca.jrc.ec.europa.eu/LCDN/developerEF.xhtml).
DESCRIPTION OF THE SYSTEM BOUNDARY (X = INCLUDED IN LCA; ND = MODULE OR INDICATOR NOT
DECLARED; MNR = MODULE NOT RELEVANT)
BENEFITS AND
CONSTRUCTI LOADS
PRODUCT STAGE ON PROCESS USE STAGE END OF LIFE STAGE BEYOND THE
STAGE SYSTEM
BOUNDARIES
7 Environmental Product Declaration Etex Building Performance NV – PROMATECT®-100 / PROMATECT®-200 /
PROMATECT®-250 / PROMAXON® Typ A
lairetam
waR
ylppus tropsnarT
gnirutcafunaM
eht
morf
tropsnarT
etis
eht
ot
etag
ylbmessA esU
ecnanetniaM
riapeR
tnemecalpeR tnemhsibrufeR
ygrene
lanoitarepO esu
retaw
lanoitarepO esu
noitcurtsnoc-eD
noitilomed tropsnarT
gnissecorp
etsaW
lasopsiD -esueR -yrevoceR -gnilcyceR laitnetop
A1 A2 A3 A4 A5 B1 B2 B3 B4 B5 B6 B7 C1 C2 C3 C4 D
X X X X X X X MNR MNR MNR X X X X X X X
RESULTS OF THE LCA - ENVIRONMENTAL IMPACT according to EN 15804+A2: 1 m² 15mm
PROMATECT®-100/200/250 and PROMAXON®-Typ A
Core Indicator Unit A1 A2 A3 A4 A5 B1 B2 B6 B7 C1 C2 C3 C4 D
GWP-total [kg CO2-Eq.] 1.46E+01.36E-13.94E+08.95E-21.43E+00.00E+00.00E+00.00E+00.00E+00.00E+08.53E-20.00E+01.89E-1-4.07E-1
GWP-fossil [kg CO2-Eq.] 1.51E+01.35E-14.90E+08.88E-2 3.62E-10.00E+00.00E+00.00E+00.00E+00.00E+08.47E-20.00E+01.94E-1-4.04E-1
GWP-biogenic [kg CO2-Eq.] -4.82E-22.13E-5-9.63E-1-1.06E-41.07E+00.00E+00.00E+00.00E+00.00E+00.00E+0-1.01E-40.00E+0-5.63E-3-1.89E-3
GWP-luluc [kg CO2-Eq.] 1.19E-3 5.35E-4 1.02E-3 7.25E-4 2.14E-40.00E+00.00E+00.00E+00.00E+00.00E+06.92E-40.00E+05.69E-4-2.67E-4
7.59E- 2.01E- 8.76E- 1.75E- 3.80E- 1.67E- 7.52E- -4.31E-
ODP [kg CFC11-Eq.] 0.00E+00.00E+00.00E+00.00E+00.00E+0 0.00E+0
10 17 13 17 11 17 16 15
AP [mol H+-Eq.] 4.86E-3 3.11E-3 4.15E-3 9.44E-5 8.57E-40.00E+00.00E+00.00E+00.00E+00.00E+09.00E-50.00E+01.38E-3-5.58E-4
EP-freshwater [kg PO4-Eq.] 1.14E-5 2.10E-7 1.65E-5 2.64E-7 1.46E-60.00E+00.00E+00.00E+00.00E+00.00E+02.51E-70.00E+03.25E-7-5.05E-7
EP-marine [kg N-Eq.] 1.21E-3 9.46E-4 1.82E-3 3.01E-5 2.77E-40.00E+00.00E+00.00E+00.00E+00.00E+02.87E-50.00E+03.58E-4-1.54E-4
EP-terrestrial [mol N-Eq.] 9.94E-3 1.04E-2 1.94E-2 3.58E-4 3.04E-30.00E+00.00E+00.00E+00.00E+00.00E+03.41E-40.00E+03.93E-3-1.66E-3
POCP [kg NMVOC-Eq.]2.93E-3 2.67E-3 5.30E-3 8.19E-5 7.64E-40.00E+00.00E+00.00E+00.00E+00.00E+07.81E-50.00E+01.09E-3-4.39E-4
ADPE [kg Sb-Eq.] 5.50E-7 7.89E-9 6.22E-7 7.87E-9 6.27E-80.00E+00.00E+00.00E+00.00E+00.00E+07.50E-90.00E+01.83E-8-6.34E-8
-
ADPF [MJ] 1.75E+11.72E+08.06E+11.18E+05.44E+00.00E+00.00E+00.00E+00.00E+00.00E+01.13E+00.00E+02.57E+0
6.81E+0
[m³ world-Eq
WDP 1.21E-1 7.13E-4 8.26E-1 8.24E-4 1.68E-10.00E+00.00E+00.00E+00.00E+00.00E+07.85E-40.00E+02.08E-2-2.94E-2
deprived]
GWP = Global warming potential; ODP = Depletion potential of the stratospheric ozone layer; AP = Acidification potential of land and water; EP =
Caption Eutrophication potential; POCP = Formation potential of tropospheric ozone photochemical oxidants; ADPE = Abiotic depletion potential for non-
fossil resources; ADPF = Abiotic depletion potential for fossil resources; WDP = Water (user) deprivation potential
RESULTS OF THE LCA - INDICATORS TO DESCRIBE RESOURCE USE according to EN 15804+A2: 1 m²
15mm PROMATECT®-100/200/250 and PROMAXON®-Typ A
Indicator Unit A1 A2 A3 A4 A5 B1 B2 B6 B7 C1 C2 C3 C4 D
PERE [MJ] 4.56E+0 5.30E-2 7.45E+0 6.80E-2 1.17E+1 0.00E+0 0.00E+0 0.00E+0 0.00E+0 0.00E+0 6.49E-2 0.00E+0 7.82E-1 -1.49E+0
PERM [MJ] 5.89E-1 0.00E+0 1.05E+1 0.00E+0 -1.04E+1 0.00E+0 0.00E+0 0.00E+0 0.00E+0 0.00E+0 0.00E+0 0.00E+0 -4.36E-1 0.00E+0
PERT [MJ] 5.15E+0 5.30E-2 1.79E+1 6.80E-2 1.23E+0 0.00E+0 0.00E+0 0.00E+0 0.00E+0 0.00E+0 6.49E-2 0.00E+0 3.46E-1 -1.49E+0
PENRE [MJ] 1.75E+1 1.72E+0 8.06E+1 1.19E+0 5.47E+0 0.00E+0 0.00E+0 0.00E+0 0.00E+0 0.00E+0 1.13E+0 0.00E+0 2.57E+0 -6.81E+0
PENRM [MJ] 0.00E+0 0.00E+0 3.43E-2 0.00E+0 -3.43E-2 0.00E+0 0.00E+0 0.00E+0 0.00E+0 0.00E+0 0.00E+0 0.00E+0 0.00E+0 0.00E+0
PENRT [MJ] 1.75E+1 1.72E+0 8.06E+1 1.19E+0 5.44E+0 0.00E+0 0.00E+0 0.00E+0 0.00E+0 0.00E+0 1.13E+0 0.00E+0 2.57E+0 -6.81E+0
SM [kg] 1.38E+1 0.00E+0 0.00E+0 0.00E+0 6.92E-1 0.00E+0 0.00E+0 0.00E+0 0.00E+0 0.00E+0 0.00E+0 0.00E+0 0.00E+0 0.00E+0
RSF [MJ] 0.00E+0 0.00E+0 0.00E+0 0.00E+0 0.00E+0 0.00E+0 0.00E+0 0.00E+0 0.00E+0 0.00E+0 0.00E+0 0.00E+0 0.00E+0 0.00E+0
NRSF [MJ] 0.00E+0 0.00E+0 0.00E+0 0.00E+0 0.00E+0 0.00E+0 0.00E+0 0.00E+0 0.00E+0 0.00E+0 0.00E+0 0.00E+0 0.00E+0 0.00E+0
FW [m³] 3.87E-3 6.21E-5 2.26E-2 7.79E-5 4.18E-3 0.00E+0 0.00E+0 0.00E+0 0.00E+0 0.00E+0 7.43E-5 0.00E+0 6.34E-4 -1.49E-3
PERE = Use of renewable primary energy excluding renewable primary energy resources used as raw materials; PERM = Use of
renewable primary energy resources used as raw materials; PERT = Total use of renewable primary energy resources; PENRE = Use of
non-renewable primary energy excluding non-renewable primary energy resources used as raw materials; PENRM = Use of non-
Caption
renewable primary energy resources used as raw materials; PENRT = Total use of non-renewable primary energy resources; SM = Use
of secondary material; RSF = Use of renewable secondary fuels; NRSF = Use of non-renewable secondary fuels; FW = Use of net fresh
water
RESULTS OF THE LCA – WASTE CATEGORIES AND OUTPUT FLOWS according to EN 15804+A2:
1 m² 15mm PROMATECT®-100/200/250 and PROMAXON®-Typ A
Indicator Unit A1 A2 A3 A4 A5 B1 B2 B6 B7 C1 C2 C3 C4 D
HWD [kg] 9.12E-5 5.26E-11 3.11E-8 6.25E-11 4.56E-6 0.00E+0 0.00E+0 0.00E+0 0.00E+0 0.00E+0 5.96E-11 0.00E+0 2.73E-10 -1.50E-9
NHWD [kg] 9.56E-2 2.22E-4 7.13E-1 1.86E-4 6.93E-1 0.00E+0 0.00E+0 0.00E+0 0.00E+0 0.00E+0 1.77E-4 0.00E+0 1.28E+1 -3.38E-3
RWD [kg] 5.05E-4 2.53E-6 5.61E-4 2.15E-6 6.90E-5 0.00E+0 0.00E+0 0.00E+0 0.00E+0 0.00E+0 2.05E-6 0.00E+0 2.69E-5 -4.83E-4
CRU [kg] 0.00E+0 0.00E+0 0.00E+0 0.00E+0 0.00E+0 0.00E+0 0.00E+0 0.00E+0 0.00E+0 0.00E+0 0.00E+0 0.00E+0 0.00E+0 0.00E+0
MFR [kg] 0.00E+0 0.00E+0 8.94E-1 0.00E+0 5.51E-2 0.00E+0 0.00E+0 0.00E+0 0.00E+0 0.00E+0 0.00E+0 0.00E+0 0.00E+0 0.00E+0
MER [kg] 0.00E+0 0.00E+0 0.00E+0 0.00E+0 0.00E+0 0.00E+0 0.00E+0 0.00E+0 0.00E+0 0.00E+0 0.00E+0 0.00E+0 0.00E+0 0.00E+0
EEE [MJ] 0.00E+0 0.00E+0 1.72E-4 0.00E+0 1.65E+0 0.00E+0 0.00E+0 0.00E+0 0.00E+0 0.00E+0 0.00E+0 0.00E+0 0.00E+0 0.00E+0
EET [MJ] 0.00E+0 0.00E+0 3.96E-4 0.00E+0 2.97E+0 0.00E+0 0.00E+0 0.00E+0 0.00E+0 0.00E+0 0.00E+0 0.00E+0 0.00E+0 0.00E+0
HWD = Hazardous waste disposed; NHWD = Non-hazardous waste disposed; RWD = Radioactive waste disposed; CRU = Components
Caption for re-use; MFR = Materials for recycling; MER = Materials for energy recovery; EEE = Exported electrical energy; EET = Exported
thermal energy
RESULTS OF THE LCA – additional impact categories according to EN 15804+A2-optional:
1 m² 15mm PROMATECT®-100/200/250 and PROMAXON®-Typ A
Indicator Unit A1 A2 A3 A4 A5 B1 B2 B6 B7 C1 C2 C3 C4 D
[Disease
PM 5.82E-8 6.05E-8 1.68E-7 6.47E-10 1.61E-8 0.00E+0 0.00E+0 0.00E+0 0.00E+0 0.00E+06.17E-100.00E+0 1.71E-8 -5.00E-9
Incidence]
[kBq U235-
IRP 5.30E-2 3.66E-4 6.95E-2 3.15E-4 8.54E-3 0.00E+0 0.00E+0 0.00E+0 0.00E+0 0.00E+0 3.00E-4 0.00E+0 2.83E-3 -7.93E-2
Eq.]
ETP-fw [CTUe] 5.20E+0 1.26E+0 5.25E+0 8.77E-1 8.15E-1 0.00E+0 0.00E+0 0.00E+0 0.00E+0 0.00E+0 8.36E-1 0.00E+0 1.46E+0-1.43E+0
-8.99E-
HTP-c [CTUh] 7.28E-102.45E-117.88E-101.77E-119.61E-110.00E+0 0.00E+0 0.00E+0 0.00E+0 0.00E+01.69E-110.00E+02.16E-10
11
HTP-nc [CTUh] 2.40E-8 1.39E-9 1.46E-8 9.21E-10 3.51E-9 0.00E+0 0.00E+0 0.00E+0 0.00E+0 0.00E+08.78E-100.00E+0 2.38E-8 -2.60E-9
SQP [-] 2.50E+1 3.01E-1 2.01E+2 4.06E-1 1.15E+1 0.00E+0 0.00E+0 0.00E+0 0.00E+0 0.00E+0 3.87E-1 0.00E+0 5.19E-1 -1.02E+0
PM = Potential incidence of disease due to PM emissions; IR = Potential Human exposure efficiency relative to U235; ETP-fw = Potential
Caption comparative Toxic Unit for ecosystems; HTP-c = Potential comparative Toxic Unit for humans (cancerogenic); HTP-nc = Potential
comparative Toxic Unit for humans (not cancerogenic); SQP = Potential soil quality index
Disclaimer 1 – for the indicator “Potential Human exposure efficiency relative to U235”.
This impact category deals mainly with the eventual impact of low dose ionizing
radiation on human health of the nuclear fuel cycle. It does not consider effects due to possible
nuclear accidents, occupational exposure nor due to radioactive waste disposal in underground
facilities. Potential ionizing radiation from the soil, from radon and from some construction materials is also not
measured by this indicator.
Disclaimer 2 – for the indicators “abiotic depletion potential for non-fossil resources”, “abiotic depletion potential
for fossil resources”, “water (user) deprivation potential, deprivation-weighted water consumption”, “potential
comparative toxic unit for ecosystems”, “potential comparative toxic unit for humans – cancerogenic”, “Potential
comparative toxic unit for humans - not cancerogenic”, “potential soil quality index”.
The results of this environmental impact indicator shall be used with care as the
uncertainties on these results are high or as there is limited experienced with the indicator.
6. LCA: Interpretation
The following graph provides information on the
relative contributions of the declared modules to
various environmental impact categories.
8 Environmental Product Declaration Etex Building Performance NV – PROMATECT®-100 / PROMATECT®-200 /
PROMATECT®-250 / PROMAXON® Typ A
It can be observed that for nearly all the impact The transport of the product to the building site (A4),
categories, the manufacturing (A3), mainly determined the installation loss and waste treatment of the
by the energy required for the production process, has packaging (A5) and the end-of-life modules (C2/C4)
a very important (25-50%) or the most important only contribute to a minor extent.
impact (>50%). Only in the impact category GWP- Since a weighted average product was declared, the
luluc, various phases contribute more equally and in variance of the LCIA results of this average product
ODP, the raw materials have the most important was compared to the impacts of the single product. It
impact. could be concluded that differences were relatively low
The pre-chains of the raw materials (A1) contribute and that the average environmental impacts show a
less than 40% in most of the impact categories and are high representativity. For example for GWP-total, the
mainly linked to impacts caused by the lime and the difference between the various products was less than
fibres. 0.4kg CO2-eq and the difference percentage between
Transport of the raw materials to site (A2), has in some the impact of the specific product and of the declared
of the impact categories such as GWP luluc, AP, EP- average is less than 4%.
marine/-terrestrial and POCP a fairly important impact
(10-25%).
7. Requisite evidence
table below having "<" means that the measurements
were below the quantification limit)
7.1 Radioactivity measurements Name Value Unit
Radioactivity measurements confirm that no other Total VOC after 28d (C6-C16)
<5 µg/m³
gamma emitters than those originating from natural Limit : 1000
radiation sources are contained. The measured R after 28d (c/NIK) <1 -
radioactivity levels do not exceed the activity Sum of VVOC after 28d (<n-C6) <5 µg/m³
concentration indices as specified by Article 3 Sum of SVOC after 28d (>n-C16)
<5 µg/m³
(Radiation Protection 112) for building products Limit : 100
following the Council Sum of cancerogenic
<1 µg/m³
Directive 96/29. Activity concentration index ≤ 2. Limit : 1
Date: 2 December 2011 Formaldehyd
Measuring agency: SCK.CEN Laboratory for Limit : 120 <3 µg/m³
Gammaspectrometry, Mol, Belgium Acetaldehyd <3 µg/m³
Protocol: Activity concentration index (ACI)
Date: 29 November 2011
Measuring agency: Eurofins Product Testing A/S,
Galten, Denmark
7.2 VOC emissions
Report number: G10210A
VOC measurements confirmed compliance with the
requirements of DIBt DIBt-communication 4/2004 in
combination with the NIK values from AgBB (March
2008) for use in the indoor environment. (values in the
9 Environmental Product Declaration Etex Building Performance NV – PROMATECT®-100 / PROMATECT®-200 /
PROMATECT®-250 / PROMAXON® Typ A
8. References
Standards
BBSR
EN 826 BBSR table "Service lives of components for life cycle
EN 826: 1996: Thermal insulating products for building assessment according to Bewertungssystem
applications - Determination of compression behaviour Nachhaltiges Bauen (BNB)" Sustainable Building
Information Portal by the Federal Ministry of Transport,
EN 1607 Building and Urban Affairs (Bundesinstitut für Bau-
EN 1607: 1996: Thermal insulating products for ,Stadt-und Raumforschung, BBSR).
building applications - Determination of tensile strength (https://www.nachhaltigesbauen.de/baustoff-
perpendicular to faces undgebaeudedaten/
nutzungsdauern-von-bauteilen.html)
EN 1608
EN 1608: 1996: Thermal insulating products for Candidate list
building applications - Determination of tensile strength Candidate List of substances of very high concern for
parallel to faces Authorisation, published on ECHA website, latest
version 19.01.2021. (https://echa.europa.eu/candidate-
EN 12467 list-table).
EN 12467: 2004: Fibre-cement flat sheets - Product
specification and test methods CPR
Construction Products Regulation, Regulation (EU) No
EN 12667 305/2011 of the European Parliament and of the
EN 12667: 2001: Thermal performance of building Council of 9 March 2011 layingdown harmonized
materials and products- Determination of thermal conditions for the marketing of construction products
resistance by means of guarded hot plate and heat and repealing Council Directive 89/106/ EEC Text with
flow meter methods. Products of high and medium EEA relevance.
thermal resistance.
DIBt-communication 4/2004
EN 13501-1 DIBt (Deutsches Institut für Bautechnik) approval
EN 13501-1:2018, Fire classification of construction guidelines for the health-related evaluation of indoor
products and building elements - Part 1: Classification construction products-2004.
using data from reaction to fire tests.
Directive 96/29
EN 15804 Council Directive 96/29/Euratom of 13 May 1996 laying
EN 15804:2012+A2:2019, Sustainability of down basic safety standards for the protection of the
construction works — Environmental Product health of workers and the general public against the
Declarations — Core rules for the product category of dangers arising from ionising radiation.
construction products.
European List of Waste
ISO 9001 2014/955/EU: Commission Decision of 18 December
UNI EN ISO 9001:2015 September 2015, Quality 2014 amending Decision 2000/532/EC on the list of
management systems - Requirements waste pursuant to Directive 2008/98/EC of the
European Parliament and of the Council.
ISO 12572 (http://data.europa.eu/eli/dec/2014/955/oj)
DIN EN ISO 12572:2001, Hygrothermal performance
of building materials and products - Determination of ETA 06/0219
water vapour transmission properties - Cup method European technical approval of PROMATECT®-100
fire protective board.
ISO 14001
UNI EN ISO 14001:2015, Environmental management ETA 07/0297
systems - Requirements with guidance for use. European technical approval of PROMATECT®-200
fire protective board.
ISO 14025
DIN EN ISO 14025:2011-10, Environmental labels and ETA 08/0161
declarations — Type III environmental declarations — European technical approval of PROMATECT®-250
Principles and procedures. fire protective board.
ISO 45001 ETA 06/0215
ISO 45001:2018, Occupational health and safety European technical approval of PROMAXON®-Tyo A
management systems — Requirements with guidance fire protective board
for use
Eurofins Product Testing A/S
Further References Eurofins Product Testing A/S, Smedeskovvej 38, 8464
Galten, Denmark. Report number: G10210A; 2011.
AgBB
Ausschuss zur gesundheitlichen Bewertung von GaBi
Bauprodukten, AgBB (eng. German Committee for GaBi Software System and Database for Life Cycle
health-related evaluation of building products. Engineering, 1992-2021, Sphera Solutions GmbH,
10 Environmental Product Declaration Etex Building Performance NV – PROMATECT®-100 / PROMATECT®-200 /
PROMATECT®-250 / PROMAXON® Typ A
Leinfelden-Echterdingen, with acknowledgement of Report according to EN 15 804+A2:2019, Version 1.0,
LBP University of Stuttgart, program version GaBi 10; Institut Bauen und Umwelt e.V., 2020.
database version 2021.1.
PCR Part B
GaBi documentation Product Category Rules for Building Products, Part B :
GaBi dataset documentation for the software system Requirements on the EPD for Calcium silicate
and databases, LBP, University of Stuttgart and insulating materials, version 1.6, 2017 www.bau-
Sphera Solutions GmbH, Leinfelden-Echterdingen, umwelt.de
2021.
(http://www.gabi-software.com/support/gabi/gabi- REACH Regulation
database-2021-lci-documentation/) Regulation (EU) No 1907/2006 of the European
Parliament and of the Council of 18 December 2006
IBU 2021 concerning the Registration, Evaluation, Authorisation
Institut Bauen und Umwelt e.V.: General Programme and Restriction of Chemicals (REACH), establishing a
Instructions for the Preparation of EPDs at the Institut European Chemicals Agency, amending Directive
Bauen und Umwelt e.V. Version 2.0, Berlin: Institut 1999/45/EC and repealing Council Regulation (EEC)
Bauen und Umwelt e.V., 2021 No 793/93 and Commission
(http://www.ibu-epd) Regulation (EC) No 1488/94 as well as Council
Directive 76/769/EEC and Commission Directives
Ordinance on Biocide Products 91/155/EEC, 93/67/EEC, 93/105/EC and 2000/21/EC.
Regulation (EU) No 528/2012 of the European
Parliament and of the Council of 22 May 2012 SCK CEN Laboratory
concerning the making available on the market and Belgian Nuclear Research Centre in Mol.
use of biocidal products.
PCR Part A
PCR Part A: Calculation rules for the Life Cycle
Assessment and Requirements on the Background
11 Environmental Product Declaration Etex Building Performance NV – PROMATECT®-100 / PROMATECT®-200 /
PROMATECT®-250 / PROMAXON® Typ A
Publisher
Institut Bauen und Umwelt e.V. Tel +49 (0)30 3087748- 0
Panoramastr. 1 Fax +49 (0)30 3087748- 29
10178 Berlin Mail info@ibu-epd.com
Germany Web www.ibu-epd.com
Programme holder
Institut Bauen und Umwelt e.V. Tel +49 (0)30 - 3087748- 0
Panoramastr 1 Fax +49 (0)30 – 3087748 - 29
10178 Berlin Mail info@ibu-epd.com
Germany Web www.ibu-epd.com
Author of the Life Cycle
Assessment Tel +32 (0)15 71 82 83
Peggy Van De Velde Fax +32 (0)15 71 82 29
Bormstraat 24 Mail
2830 Tisselt peggy.vandevelde@etexgroup.c
Belgium om
Web www.etexgroup.com
Owner of the Declaration
Etex Building Performance Tel +32 2 778 12 11
International Fax +32 2 778 12 12
Rue Marcel Demonque 500 r Mail info@etexgroup.com
84915 Avignon Cedex 9 Web http://www.etexgroup.com
France
