ENVIRONMENTAL PRODUCT DECLARATION
as per ISO 14025 and EN 15804+A2
Owner of the Declaration INDURA
Publisher Institut Bauen und Umwelt e.V. (IBU)
Programme holder Institut Bauen und Umwelt e.V. (IBU)
Declaration number EPD-IND-20230122-CBC1-EN
Issue date 14.06.2023
Valid to 13.06.2028
Flanges and butt welded fittings
INDURA
www.ibu-epd.com | https://epd-online.com
General Information
INDURA Flanges and butt welded fittings
Programme holder Owner of the declaration
IBU – Institut Bauen und Umwelt e.V. INDURA
Hegelplatz 1 Grønlandsvej 1
10117 Berlin 7480 Vildbjerg
Germany Denmark
Declaration number Declared product / declared unit
EPD-IND-20230122-CBC1-EN 1 kilogram of flange or butt welded fitting in carbon steel or galvanized
steel
This declaration is based on the product category rules: Scope:
Steel pipes for pressure applications, 01.08.2021 A life cycle assessment according to ISO 14040/44 has been conducted
(PCR checked and approved by the SVR) individually for 1 kg (worst-case product) of the three product groups:
• Flanges of carbon steel
• Flanges of galvanized steel
Issue date
• Butt welded fittings of carbon steel
14.06.2023
Due to the variations in products and production locations, the worst-case
EPD approach has been applied and the highest environmental impacts
Valid to have been declared.
13.06.2028
The materials and metal shaping processes originate from a multitude of
suppliers which INDURA is not in operational control over. The suppliers'
locations are mainly China, but also Vietnam, Cambodia, Slovakia,
Romania, and Germany. A conservative average approach has been
applied to make the EPD representative for the many suppliers from
different locations, thus Chinese and Asian representative data is applied
to the calculation in terms of the energy mix and transport distances.
INDURAs own facility is located in Vildbjerg, Denmark and emissions from
that location are modelled with Danish energy mixes.
The owner of the declaration shall be liable for the underlying information
Dipl.-Ing. Hans Peters and evidence; the IBU shall not be liable with respect to manufacturer
(Chairman of Institut Bauen und Umwelt e.V.) information, life cycle assessment data and evidences.
The EPD was created according to the specifications of EN 15804+A2. In
the following, the standard will be simplified as EN 15804.
Verification
The standard EN 15804 serves as the core PCR
Independent verification of the declaration and data according to ISO
14025:2011
internally X externally
Dipl.-Ing. Hans Peters Dr.-Ing. Nikolay Minkov,
(Managing Director Institut Bauen und Umwelt e.V.) (Independent verifier)
1 Environmental Product Declaration - INDURA - Flanges and butt welded fittings
Product
• EN10025-2
Product description/Product definition • BS EN 10025-2:2019
This EPD includes the following products depending on • EN10222-1
application for oil, gas and water pipe systems: • EN10222-2
• flanges in carbon steel (also referred to as black steel) • EN10222-4
or galvanized steel (hot dip galvanized) • EN10028-1
• butt welded fittings in carbon steel (also referred to as • EN10028-2
black steel) • EN10028-6
The products covered in this EPD are classified and traded • DIN 2501
under the following TARif Intégré Communautaire (TARIC) • DIN 2519
codes: 7307931199, 7307931999, 7307939190, and • DIN 2527
7307910090. • DIN 2566
This EPD specifically excludes the following products: • DIN 2573
• DIN 2576
• products in stainless steel
• DIN 2632
• flange gaskets
• DIN 2633
• threaded fittings
• DIN 2634
• valves.
• DIN 2635
• DIN 2641
For the placing on the market in the European Union/European
• DIN 2642
Free Trade Association (EU/EFTA) (with the exception of
• DIN 2673
Switzerland) the following legal provisions apply: 2014/68/EU of
• DIN 28461
the European Parliament and of the Council of 15 May 2014 on
• DIN 86030
the harmonization of the laws of the Member States relating to
• DIN 86044
the making available on the market of pressure equipment and
• ASTM A105/A105M
the harmonized standards based on these provisions:
Butt welded fittings of carbon steel follow a range of standards
• EN 1092-1:2018, Flanges and their joints – Circular in relation to materials, production and technical properties,
flanges for pipes, valves, fittings and accessories, PN depending on the type of fittings. The following standards are
designated – Part 1: Steel flanges relevant for Indura's fittings:
• EN 10253-1:2000, Butt-welding pipe fittings – Part 1:
• EN 10253-1
Wrought carbon steel for general use and without
• EN 10253-2
specific inspection requirements
• EN 10217-1
• EN 10253-2:2021, Butt-welding pipe fittings – Part 2:
• EN 10217-2
Non alloy and ferritic alloy steels with specific inspection
• EN 10217-3
requirements
• EN 10217-4
The CE-marking takes into account the proof of conformity with
• EN 10216-1
the respective harmonized standards based on the legal
• EN 10216-2
provisions above. For the application and use the respective
• EN ISO 3183
national provisions apply.
• ASME B16.9
Application • ASTM A234
• DIN 2618
Flanges and butt welded fittings are used to connect different
• DIN 2619
pipes with each other and can be used both for transporting oils
• DIN 2642
and in connection with water. The flanges are usually in the
• DIN 28011
form of an annular disc and are attached to the end of a pipe,
where screws and nuts are used to secure the flange and Constructional data
connect the pipes. The different types of flanges include Name Value Unit
threaded flanges, blind flanges, welding ring flanges, loose
Yield strength 235 - 355 N/mm2
flanges, welding neck flanges, welding neck collars.
Tensile strength 360 - 655 N/mm2
Butt welded fittings have no threads, which means that they Elongation min. 14 - 30 1
can only be permanently connected by means of a weld. Butt Hardness 114-197 HV
welded fittings cover different types of fittings in various shapes
Notched-bar impact value min. 20-27 Joule
and dimension, such as pipe bends, tees, crosses, welded
Ductility min. 14-25 %
elbows, saddle elbows, concentric reducers, and excentric
reducers. Performance data of the product in accordance with the
declaration of performance with respect to its essential
Technical Data characteristics according to
Flanges of carbon steel and galvanized steel follow a range of
• EN 1092-1:2018, Flanges and their joints – Circular
standards in relation to materials, production and technical
flanges for pipes, valves, fittings and accessories, PN
properties, depending on the type of flanges. The following
designated – Part 1: Steel flanges.
standards are relevant for Indura's flanges:
• EN 10253-1:2000, Butt-welding pipe fittings – Part 1:
• EN1092-1 Wrought carbon steel for general use and without
• ASME B16.5 specific inspection requirements.
• ASME B16.47
• JIS B2220
• EN10025-1
2 Environmental Product Declaration - INDURA - Flanges and butt welded fittings
mesh.
Base materials/Ancillary materials This product/article/at least one partial article contains
Main material constituents per 1 kg of product in delivery status. substances listed in the candidate list exceeding 0.1
Name Value Unit percentage by mass: no.
This product/article/at least one partial article contains other
Steel 97.8 %
carcinogenic, mutagenic, reprotoxic (CMR) substances in
Zinc for galvanization 2.1 %
categories 1A or 1B which are not on the candidate list,
Rust protection naphtha oil 0.1 %
exceeding 0.1 percentage by mass: no.
The flanges and butt welded fittings are produced in carbon Biocide products were added to this construction product or it
steel, following the material norms EN 10222-2 and EN 10028- has been treated with biocide products (this then concerns a
2. treated product as defined by the (EU) Ordinance on Biocide
The main material constituents in the table above are based on Products No. 528/2012): no.
the product in delivery status. However, the input of steel varies
Reference service life
for the 3 different product groups that are declared. For flanges
in carbon steel, the steel input is 1.80 kg, for galvanized flanges The life cycle of steel flanges and butt welded fittings is
the steel input is 1.78 kg, for the fittings in carbon steel the dependent on the respective structural design, use and
material input is 1.08 kg steel. Additionally, various packaging maintenance. The use phase for steel pipe for oil and gas
materials are also calculated per declared unit. This includes pipelines is not depicted as they involve maintenance-free and
25*10^-7 kg PVC tape, 0.15 kg cardboard, 0.0011 kg wood generally durable products. The reference service life is not
EUR pallet, and 0.0027 kg high density polyethylene (HDPE) declared, as the use phase is not included in the scope.
LCA: Calculation rules
Declared Unit
The declared unit is 1 kg of flange or butt welded fitting in
carbon steel or galvanized steel, where the highest of each
LCIA result is declared on the final EPD.
Declared unit and mass reference
Name Value Unit
Declared unit 1 kg
Conversion factor to metric tonne 1000 -
System boundary
Type of EPD: cradle to gate with Modules C1–C4 and Module
D.
The product stage (modules A1-A3) consists of raw material
extraction and processing (A1) as well as the transport to the
manufacturing location (A2) and activities at the manufacturing
facility (A3). In this study, the processes A1-A3 are all included.
Wastes and losses of manufacturing processes are included in
the unit processes in which they occur according to the polluter
pays principle and the modular approach of EN 15804.
The product stages (A1 and A3) for flanges can be seen above.
Practically this means that the metal scrap is modelled so that
its waste processing is included in A3 and credited by reducing
the input in A1 to the net consumption of steel. However, this
credit cannot exceed the input of secondary metals based on a
market average. According to the American Iron and Steel
Institute (American Iron and Steel Institute, 2012) the average
recycled content of steel is 36.9 % when it originates from basic
oxygen furnaces. However, for electric arc furnaces, the
recycled content is 89.9 %. The sourced materials from Asia
that INDURA purchases are most likely originating from basic
oxygen furnaces, but the steel market is constrained (all
available ferrous metal is generally recycled). For this reason, a
total average of the steel recycled
content should be applied. It is decided that a conservative
approach is used in the calculation and the net input of steel is
then modelled as primary (virgin) steel.
3 Environmental Product Declaration - INDURA - Flanges and butt welded fittings
as metal. 5 % are considered lost during the recycling process
and are modelled as inert material landfilling. End-of-life
treatment of the packaging is not included in the study.
Benefits and loads beyond the system boundaries (module
D) include the potential benefits from reuse, recycling and
recovery potentials that are outside the scope of the study. This
would include all the flows leaving the product system having
passed the end-of-waste stage, thereby allowing the use of
them as a substitution for primary material in another product
system. Thus, the system will get credit for recycling the
collected steel. 5 % are considered lost in the sorting process,
thus 95 % of the product is credited in module D.
As the steel scrap from production processes is credited in the
A1-A3 modules, only the end-of-life product will be credited in
module D. The scrap should however first reach functional
equivalence to steel, which requires it to be processed using an
electric arc furnace (EAF) process. The system is then credited
with the avoided production of virgin steel produced using the
basic oxygen furnace (BOF) process.
Geographic Representativeness
Land or region, in which the declared product system is
manufactured, used or handled at the end of the product´s
lifespan: Denmark
The product stages (A1 and A3) for butt welded fittings can be
seen above. Comparability
Basically, a comparison or an evaluation of EPD data is only
At the end-of-life stage (module C1-C4), INDURAs products
possible if all the data sets to be compared were created
are assumed to be manually disassembled from the piping
according to EN 15804 and the building context, respectively
system in which it has been installed. As a result, no processes
the product-specific characteristics of performance, are taken
have been added to the C1 module. Most customers (>93%)
into account. Furthermore, in order to ensure comparability
are located in Northern Europe (Scandinavia, Germany and
between EPDs background databases should be consistent.
Benelux), thus the transportation distances, technology and
For this declaration, ecoinvent v3.9 has been used.
waste processing will be modelled accordingly. For the waste
processing, it is assumed that the product itself will be recycled
LCA: Scenarios and additional technical information
End of life (C1-C4)
Characteristic product properties of biogenic carbon
The biogenic carbon content in the flanges or fittings leaving Name Value Unit
the factory gate is 0 %. Collected separately 1 kg
The biogenic carbon content in the accompanying packaging is Recycling 0.95 kg
46 %, as it mainly consists of cardboard and wood pallet.
Landfilling 0.05 kg
Information on describing the biogenic Carbon Content at
factory gate Reuse, recovery and/or recycling potentials (D), relevant
scenario information
Name ValueUnit
Name Value Unit
kg
Biogenic carbon content in product 0 C Collection rate 95 %
Biogenic carbon content in accompanying kg EoL amount 0.590 kg
0.07
packaging C 5 % losses are assumed in the sorting and recycling system.
This study is a Model EPD where the worst-case scenarios are
Packaging is included and declared in module A3. However, declared. As a result, module D declares the lowest possible
since module A5 is not declared in this EPD, the disposal of the recycling credit when compared across the three main product
packaging material on the construction site is shown below groups.
including waste amounts and the respective waste scenarios.
Per declared unit (1 kg) the following packaging wastes occur: Only the net production of steel scrap is credited for, meaning
that the consumption of secondary steel in A1 is subtracted
• Tape of PVC: 0.00003 kg assumed for landfilling
before calculating the credit in module D. The loads associated
• Cardboard box: 0.150 kg assumed for recycling
with the processing of steel scrap must have functional
• EUR-pallet of wood: 0.0011 kg assumed for incineration
equivalence with steel produced from virgin sources. This is
• Mesh netting of HDPE: 0.0027 kg assumed for
done through an electric arc furnace process (EAF) process.
recycling.
The amount of steel produced from the collected scrap steel is
then credited with the production of steel from virgin sources,
using a basic oxygen furnace (BOF) process.
4 Environmental Product Declaration - INDURA - Flanges and butt welded fittings
LCA: Results
DESCRIPTION OF THE SYSTEM BOUNDARY (X = INCLUDED IN LCA; ND = MODULE OR INDICATOR NOT DECLARED; MNR =
MODULE NOT RELEVANT)
Benefits and
Construction loads beyond
Product stage Use stage End-of-life stage
process stage the system
boundaries
la ire ta m w a Ry lp p u s tro p s n a rT g n iru tc a fu n a M e h t m o rf tro p s n a rTe tis e h t o t e ta g y lb m e s s A e s U e c n a n e tn ia M ria p e R tn e m e c a lp e R tn e m h s ib ru fe R y g re n e la n o ita re p Oe s u re ta w la n o ita re p Oe s u n o itc u rts n o c -e Dn o itilo m e d tro p s n a rT g n is s e c o rp e ts a W la s o p s iD -e s u e R-y re v o c e R-g n ilc y c e Rla itn e to p
A1 A2 A3 A4 A5 B1 B2 B3 B4 B5 B6 B7 C1 C2 C3 C4 D
X X X MND MND MND MND MNR MNR MNR MND MND X X X X X
RESULTS OF THE LCA - ENVIRONMENTAL IMPACT according to EN 15804+A2: 1 kg flange or butt welded fitting of carbon
steel or galvanized steel
Parameter Unit A1-A3 C1 C2 C3 C4 D
Global Warming Potential total (GWP-total) kg CO 2 eq 5.69E+00 0 4.18E-03 2.21E-02 3.08E-04 -1.11E+00
Global Warming Potential fossil fuels (GWP-fossil) kg CO 2 eq 5.66E+00 0 4.18E-03 2.25E-02 3.07E-04 -1.11E+00
Global Warming Potential biogenic (GWP-biogenic) kg CO 2 eq 2.03E-02 0 3.31E-06 -4.64E-04 1.61E-07 4.36E-03
Global Warming Potential luluc (GWP-luluc) kg CO 2 eq 1.47E-02 0 2.04E-06 2.72E-05 1.86E-07 -2.06E-04
Depletion potential of the stratospheric ozone layer (ODP) kg CFC11 eq 9.67E-08 0 9.16E-11 3.54E-10 8.9E-12 -2.4E-08
Acidification potential of land and water (AP) mol H+ eq 3.07E-02 0 1.95E-05 2.72E-04 2.32E-06 -4.65E-03
Eutrophication potential aquatic freshwater (EP-freshwater) kg P eq 2.24E-03 0 3.01E-07 1.49E-05 2.56E-08 -5.03E-04
Eutrophication potential aquatic marine (EP-marine) kg N eq 8.12E-03 0 7.75E-06 6.07E-05 8.9E-07 -1.05E-03
Eutrophication potential terrestrial (EP-terrestrial) mol N eq 7.67E-02 0 8.29E-05 6.79E-04 9.53E-06 -1.13E-02
Formation potential of tropospheric ozone photochemical oxidants kg NMVOC
2.88E-02 0 2.89E-05 2.01E-04 3.32E-06 -5.96E-03
(POCP) eq
Abiotic depletion potential for non fossil resources (ADPE) kg Sb eq 7.06E-05 0 1.33E-08 1.59E-06 4.33E-10 -9.75E-06
Abiotic depletion potential for fossil resources (ADPF) MJ 6.58E+01 0 6.07E-02 3.07E-01 7.71E-03 -1.03E+01
m3 world eq
Water use (WDP) 2.14E+00 0 3.08E-04 5.46E-03 2.4E-05 -1.86E-01
deprived
RESULTS OF THE LCA - INDICATORS TO DESCRIBE RESOURCE USE according to EN 15804+A2: 1 kg flange or butt welded
fitting of carbon steel or galvanized steel
Parameter Unit A1-A3 C1 C2 C3 C4 D
Renewable primary energy as energy carrier (PERE) MJ 5E+00 0 9.53E-04 5.36E-02 6.48E-05 -7.15E-01
Renewable primary energy resources as material utilization
MJ 2.17E+00 0 0 0 0 0
(PERM)
Total use of renewable primary energy resources (PERT) MJ 7.17E+00 0 9.53E-04 5.36E-02 6.48E-05 -7.15E-01
Non renewable primary energy as energy carrier (PENRE) MJ 6.55E+01 0 6.07E-02 3.07E-01 7.71E-03 -1.03E+01
Non renewable primary energy as material utilization (PENRM) MJ 3.28E-01 0 0 0 0 0
Total use of non renewable primary energy resources (PENRT) MJ 6.58E+01 0 6.07E-02 3.07E-01 7.71E-03 -1.03E+01
Use of secondary material (SM) kg 7.96E-01 0 2.7E-05 3.42E-04 1.86E-06 7.82E-01
Use of renewable secondary fuels (RSF) MJ 1.75E-02 0 3.34E-07 1.72E-05 3.99E-08 -8.44E-05
Use of non renewable secondary fuels (NRSF) MJ 0 0 0 0 0 0
Use of net fresh water (FW) m3 2.32E-02 0 7.73E-06 1.56E-04 7.97E-06 -2.01E-03
RESULTS OF THE LCA – WASTE CATEGORIES AND OUTPUT FLOWS according to EN 15804+A2:
1 kg flange or butt welded fitting of carbon steel or galvanized steel
Parameter Unit A1-A3 C1 C2 C3 C4 D
Hazardous waste disposed (HWD) kg 6.23E-01 0 4.08E-05 8.24E-04 3.7E-06 -1.64E-01
Non hazardous waste disposed (NHWD) kg 8.04E+00 0 1.27E-03 5.85E-02 1.11E-04 -1.98E+00
Radioactive waste disposed (RWD) kg 1.77E-05 0 4.97E-09 1.66E-07 3.24E-10 2.49E-06
Components for re-use (CRU) kg 0 0 0 0 0 0
Materials for recycling (MFR) kg 5.14E-01 0 4.57E-07 1E+00 3.46E-08 -6.79E-05
Materials for energy recovery (MER) kg 5.56E-05 0 2.82E-09 4.63E-08 1.24E-10 -5.95E-06
Exported electrical energy (EEE) MJ 2.13E-02 0 1E-05 3.75E-04 4.24E-07 1.11E-02
Exported thermal energy (EET) MJ 2.64E-02 0 2.37E-05 5.76E-05 2.64E-07 -9.6E-03
RESULTS OF THE LCA – additional impact categories according to EN 15804+A2-optional:
1 kg flange or butt welded fitting of carbon steel or galvanized steel
Parameter Unit A1-A3 C1 C2 C3 C4 D
Disease
Incidence of disease due to PM emissions (PM) 4.62E-07 0 4.11E-10 3.65E-09 5.07E-11 -7.65E-08
incidence
Human exposure efficiency relative to U235 (IR) kBq U235 eq 2.42E-01 0 8.34E-05 2.74E-03 4.85E-06 5.38E-02
5 Environmental Product Declaration - INDURA - Flanges and butt welded fittings
Comparative toxic unit for ecosystems (ETP-fw) CTUe 4.14E+01 0 2.95E-02 2.37E-01 3.58E-03 -1.85E+00
Comparative toxic unit for humans (carcinogenic) (HTP-c) CTUh 3.08E-08 0 2.33E-12 4.19E-11 1.38E-13 9.95E-09
Comparative toxic unit for humans (noncarcinogenic) (HTP-nc) CTUh 1.16E-07 0 4.71E-11 1.75E-09 1.65E-12 -8.18E-09
Soil quality index (SQP) SQP 3.19E+01 0 4.53E-02 5.87E-01 1.52E-02 -3.25E+00
Disclaimer 1 – for the indicator 'Potential Human exposure efficiency relative to U235'. This impact category deals mainly with the
eventual impact of low-dose ionizing radiation on human health of the nuclear fuel cycle. It does not consider effects due to possible
nuclear accidents, occupational exposure or radioactive waste disposal in underground facilities. Potential ionizing radiation from the
soil, radon and from some construction materials is also not measured by this indicator.
Disclaimer 2 – for the indicators 'abiotic depletion potential for non-fossil resources', 'abiotic depletion potential for fossil resources',
'water (user) deprivation potential, deprivation-weighted water consumption', 'potential comparative toxic unit for ecosystems', 'potential
comparative toxic unit for humans – cancerogenic', 'Potential comparative toxic unit for humans - not cancerogenic', 'potential soil
quality index'. The results of this environmental impact indicator shall be used with care as the uncertainties on these results are high
as there is limited experience with the indicator.
References
Standards low temperature properties.
ASTM A234 EN 10217-4
ASTM A234/A234M - 22, Standard Specification for Piping Welded steel tubes for pressure purposes – Technical delivery
Fittings of Wrought Carbon Steel and Alloy Steel for Moderate conditions – Part 4: Electric welded non-alloy steel tubes with
and High Temperature Service. specified low temperature properties.
ASME B16.47 EN 10253-1
B16.47 - 2020, Large Diameter Steel Flanges: NPS 26 through Butt-welding pipe fittings – Part 1: Wrought carbon steel for
NPS 60, Metric/Inch Standard. general use and without specific inspection requirements.
ASME B16.5 EN 10253-2
B16.5 - 2020, Pipe Flanges and Flanged Fittings: NPS 1/2 Butt-welding pipe fittings – Part 2: Non alloy and ferritic alloy
through NPS 24, Metric/Inch Standard. steels with specific inspection requirements.
ASME B16.9 EN ISO 3183
B16.9 - 2018, Factory-Made Wrought Buttwelding Fittings Petroleum and natural gas industries – Steel pipe for pipeline
BS EN 10025 transportation systems (ISO 3183:2019).
BS EN 10025-2:2019, hot rolled products of structural steel. ISO 14025
Documents provided by IBU: Environmental labels and declarations — Type III
Product Category Rules for Building-Related Products and environmental declarations — Principles and procedures.
Services: Part A: Calculation Rules for the Life Cycle JIS B 2220
Assessment and Requirements on the Project Report according JIS B 2220:2004, Steel pipe flanges.
to EN 15804+A2:2019 version 1.3 Further references
Product Category Rules Part B: Requirements on the EPD for American Iron and Steel Institute. (2012).
Steel pipes for pressure applications 01/08/2021 (version 1). CSSBI. From
EN 15804 https://cssbi.ca/assets/resources/Enviro_Fact_Sheet/SRILEED_Recycled-
EN 15804+A2:2019, Sustainability of construction works — ontent.pdf [access on 10-12-2022]
Environmental Product Declarations — Core rules for the Candidate List of Substances of Very High Concern
product category of construction products. https://echa.europa.eu/candidate-list-table [access on 12-06-
EN ISO 14040/44 23]
EN ISO 14040:2006, Environmental management – Life cycle EcoInvent 3.9
assessment - Principles and framework; English version EN EcoInvent database version 3.9, cut-off, EN15804 model. LCIA
ISO 14040:2006 EN ISO 14044:2006, Environment methodology EF v3.1 EN15804. Wernet, G., Bauer, C.,
Management – Life Cycle Assessment – Requirements and Steubing, B., Reinhard, J., Moreno-Ruiz, E., and Weidema, B.,
Instructions; English version EN ISO 14044:2006. 2016. The ecoinvent database version 3 (part I): overview and
EN 1092-1 methodology. The International Journal of Life Cycle
Flanges and their joints – Circular flanges for pipes, valves, Assessment.
fittings and accessories, PN designated – Part 1: Steel flanges. IBU 2021
EN 10216-2 Institut Bauen und Umwelt e.V.: General Instructions for the
Seamless steel tubes for pressure purposes – Technical EPD programme of Institut Bauen und Umwelt e.V., Version
delivery conditions – Part 2: Non-alloy and alloy steel tubes with 2.0, Berlin: Institut Bauen und Umwelt e.V., 2021 www.ibu-
specified elevated temperature properties. epd.com
EN 10217-1 INDURA
Welded steel tubes for pressure purposes – Technical delivery https://www.indura.com/products [access on 10-12-22]
conditions – Part 1: Electric welded and submerged arc welded Ordinance on Biocide Products No. 528/2012
non-alloy steel tubes with specified room temperature Regulation (EU) No 528/2012 of the European Parliament and
properties. of the Council of 22 May 2012 concerning the making available
EN 10217-2 on the market and use of biocidal products Text with EEA
Welded steel tubes for pressure purposes – Technical delivery relevance.
conditions – Part 2: Electric welded non-alloy and alloy steel SimaPro 2023
tubes with specified elevated temperature properties. LCA Software; PRé Sustainability, Version 9.5
EN 10217-3 TARIC
Welded steel tubes for pressure purposes – Technical delivery TARIC, the integrated Tariff of the European Union.
conditions – Part 3: Electric welded and submerged arc welded https://ec.europa.eu/taxation_customs/dds2/taric/taric_consultation.jsp?
alloy fine grain steel tubes with specified room, elevated and ang=en [access on 12-06-23]
6 Environmental Product Declaration - INDURA - Flanges and butt welded fittings
Publisher
Institut Bauen und Umwelt e.V. +49 (0)30 3087748- 0
Hegelplatz 1 info@ibu-epd.com
10117 Berlin www.ibu-epd.com
Germany
Programme holder
Institut Bauen und Umwelt e.V. +49 (0)30 3087748- 0
Hegelplatz 1 info@ibu-epd.com
10117 Berlin www.ibu-epd.com
Germany
Author of the Life Cycle Assessment
Viegand Maagøe +4533349000
Nørre Farigmagsgade 37 info@viegandmaagoe.dk
1364 Copenhagen www.viegandmaagoe.dk/en
Denmark
Owner of the Declaration
INDURA +45 97133244
Grønlandsvej 1 salg@indura.dk
7480 Vildbjerg www.indura.dk/
Denmark
7 Environmental Product Declaration - INDURA - Flanges and butt welded fittings
