ENVIRONMENTAL PRODUCT DECLARATION
as per /ISO 14025/ and /EN 15804/
Owner of the Declaration Etex Building Performance International
Programme holder Institut Bauen und Umwelt e.V. (IBU)
Publisher Institut Bauen und Umwelt e.V. (IBU)
Declaration number EPD-ETX-20190099-IBA1-EN
Issue date 08.01.2020
Valid to 07.01.2025
BLUCLAD
Fibre cement backerboard for render- & (brick)slipsystems
Etex Building Performance International
www.ibu-epd.com / https://epd-online.com
Umwelt Produktdeklaration Name des Herstellers – Name des Produkts
1. General Information
Etex Building Performance International Bluclad
Programme holder Owner of the declaration
IBU - Institut Bauen und Umwelt e.V. Etex Building Performance International
Panoramastr. 1 500 rue Marcel Demonque
10178 Berlin 84915 Avignon Cedex 9
Germany FRANCE
Declaration number Declared product / declared unit
EPD-ETX-20190099-IBA1-EN 1 m² Bluclad
This declaration is based on the product Scope:
category rules: The Environmental Product Declaration includes the
Fibre cement / Fibre concrete, 07.2014 environmental parameters for the Bluclad fibre cement
(PCR checked and approved by the SVR) backer board for render- & (brick)slip systems
produced by Etex Building Performance International.
The result of the life cycle assessment is based on a
Issue date
thickness of 10 mm. This document refers to the
08.01.2020
structural panels manufactured in the Kapelle-op-den-
Bos plant (Belgium). The production data used refers
Valid to to production year 2016. Based on plausible,
07.01.2025 transparent and comprehensible basic data, the Life
Cycle Assessment fully represents the Etex products in
question.
The owner of the declaration shall be liable for the
underlying information and evidence; the IBU shall not
be liable with respect to manufacturer information, life
cycle assessment data and evidences.
Verification
The standard /EN 15804/ serves as the core PCR
Independent verification of the declaration and data
according to /ISO 14025:2010/
Dipl. Ing. Hans Peters internally x externally
(President of Institut Bauen und Umwelt e.V.)
Dr. Alexander Röder Dipl. Natw. ETH Sascha Iqbal
(Head of Board IBU) (Independent verifier appointed by SVR)
2. Product
2.1 Product description / Product definition Federal Institute for Materials Research and Testing
This Environmental Product Declaration refers to large- (/BAM/).
format structural cellulose-reinforced fibre cement
panels. The products under review involve smooth For the application and the use the respective national
panels made from steam-hardened fibre cement. provisions apply.
For the placing on the market of the product in the 2.2 Application
European Union / European Free Trade Association Bluclad fibre cement boards serve as a backer-board
(EFTA) (with the exception of Switzerland) the for render systems or finishing with slips (brick slips,
/Construction Products Regulation/ applies. The mineral stripes, natural or concrete slips, tiles, …)
product needs a declaration of performance taking into within ventilated façade applications or external
consideration /EN 12467/: Fibre-cement flat sheets - ceilings. Within ventilated facades, the boards are fixed
Product specification and test methods. in wooden studs or steel studs, applied on massive
construction (blocks, concrete, limestone, …) or light-
CE Declaration of Conformity in accordance with the weight wood frame or steel frame. As a non-ventilated
specifications outlined in Annex ZA to /EN 12467/. façade, Bluclad can be applied on wood- & steelframe.
General technical approval no. /Z-31.4-160/ of the All relevant details are prescribed in the design &
"Deutsches Institut für Bautechnik" (DIBt). application guidelines.
External monitoring of the products with general 2.3 Technical Data
technical approval by the Material Testing Institute of Standard-related tests for CE marking via type testing
the state of Brandenburg/Berlin and the German in accordance with /EN 12467/.
2 Environmental Product Declaration ETEX – Bluclad Plaster Base Boards
This product contains other carcinogenic, mutagenic
Constructional data and toxic for reproduction (CMR) substances in
Name Value Unit categories 1A or 1B which are not on the candidate
Gross density dry, mean, +/- 10% 1180 kg/m3 list, exceeding 0.1 percentage by mass: no
Compressive strength 38 N/mm2
Modulus of elasticity perpendicular >7.5 N/mm2 Biocide products were added to this construction
Modulus of elasticity parallel >8.5 N/mm² product or it has been treated with biocide products
Flexural strength perpendicular >10.4 N/mm2 (this then concerns a treated product as defined by the
Flexural strength parallel >16.9 N/mm² (EU) /Ordinance on Biocide Products/): no
Tensile strength 6.3 N/mm2
2.6 Manufacture
Water vapour diffusion resistance 84 (wet) -
- Large-format panels made of fibre cement are
factor 143 (dry)
manufactured mainly in accordance with an automated
Moisture content at 23 °C, 80%
6 M.-% winding process. The raw materials are treated with
humidity
water to form a homogeneous mixture. Rotating screen
Coefficient of thermal expansion <6.5 10-6K-1
cylinders are immersed in this fibre cement pulp which
Swelling (air-dry to water-
7 mm/m drains the mixture outwards. The screen surface is
saturated)
coated with a thin fibre cement film which is conveyed
similar to
onto an infinite transport belt from where it reaches a
Chemical resistance concrete -
format roller to which an increasingly thick layer of fibre
C35/C45
cement is applied.
similar to
Once the requisite material thickness has been
Ageing resistance concrete -
achieved, the still moist and malleable fibre cement
C35/C45
layer (fibre cement fleece) is unravelled and detached
Permanent temperature
up to 100 °C from the format roller.
resistance
The fibre cement fleece is cut to length and any
Thermal conductivity 0.19 W/(mK)
leftovers are returned to the production process with
the result that no waste is incurred. The panels are
then set aside for binding before stacking on pallets
Performance data of the product in accordance with and steam-hardened in an autoclave for approx. 2
the declaration of performance with respect to its hours. The setting time lasts approx. 3 days.
essential characteristics according to /EN 12467/. The Bluclad boards are then hydrophobised (water-
repellent finish). The hydrophobic finish is applied
2.4 Delivery status using roller technology. The excess hydrophobic fluid
The Bluclad is delivered with a maximum size of 3.100 is collected in full and redirected into the production
mm x 1.500 mm and a thickness of 10 mm. The process.
surface has a slight waffle structure with a hydrophobic
finish. The production facilities are certified in accordance
with /ISO 9001/.
2.5 Base materials / Ancillary materials
Base materials in % mass (dry mass): 2.7 Environment and health during
 25-45% Portland cement to /EN 197-1/, (CEM manufacturing
I 32.5 R and 42.5 R) (binding agent) During the entire manufacturing process, there are no
 25-45% Quartz sand, mineral aggregates other health protection measures extending beyond
the legally specified industrial protection measures for
 1-15% Wollastonite
commercial enterprises.
 1-10% Cellulose fibres
 Air: Any dust incurred is collected in filter
 1-10% Mica
systems and partially re-used. Emissions are
 1-10% Aluminium hydroxide
significantly lower than the limit values
specified by the TA Air.
and water for mixing the cement: 0.24 m³/t fibre  Water/Soil: Water incurred during
cement.
manufacturing and plant cleaning is treated
mechanically in waste water treatment
Water-repellent finish
systems on the plant site and re-used in the
Application volume 80 g/m²
The water-repellency is obtained through the production process.
introduction of organosilanes on the surface of the  Noise: The noise emissions into the
board. environment by production equipment fall
Cellulose-reinforced fibre cement products were
short of the permissible limit values.
introduced in 1980s as a safe replacement for the
widely used asbestos cement products manufactured
before that time. The production facilities are certified in accordance
Information that product does not contain substances with /ISO 14001/ and /OHSAS 18001/.
listed in the Candidate List of substances of very high
concern (/REACH Regulation/) exceeding 0.1%: 2.8 Product processing/Installation
This product contains substances listed in the Special low-dust equipment such as slow-running,
candidate list (date: 15.01.2019) exceeding 0.1 carbide-tipped splitting saws or cutting burs are
percentage by mass: no available for processing. Drill holes can be made using
standard high-speed steel twist (HSS) drills. Additional
products required for installing the products under
3 Environmental Product Declaration ETEX – Bluclad Plaster Base Boards
review include: wood or metal substructures including Building materials classification to /EN 13501-1/ A2,
the requisite anchoring and joining components as well s1-d0, i.e. limited combustibility in accordance with
as securing parts (screws, nails, staples). When Part A of the Building Rules List.
selecting any requisite constructive products, please
ensure that they do not have a negative influence on Development of smoke/smoke density: smoke
the designated function of the construction products development caused by burning the products in
referred to. question (coating) is very low.
The set of rules laid out by the employers' liability
insurance associations shall apply. Combustion gases: the results in line with testing to
When processing the products under review, /DIN 53436/ indicate that the gaseous emissions
conventional industrial protection measures must be incurred when burning the panels in question are free
observed in accordance with the information supplied of sulphur and chlorine compounds. The concentration
by the manufacturer. Please note that dust generated of released hydrogen cyanide (HCN) is within a normal
during processing can have an alkaline reaction (pH framework.
value: >10).
According to the present state of knowledge, hazards Changing the system condition (burning dripping/falling
for water, air and soil cannot arise when fibre cement material): when surrounding construction materials are
is processed as designated. burned, the cellulose fibres bound in the cement
gradually lose their strength: This does not represent
2.9 Packaging any explosive potential with the result that fibre cement
Cardboard boxes, wooden pallets and steel bands are does not pose a risk in the event of a fire. Burning
used as packaging materials. The wooden pallets can dripping/falling hydrophobic treatment or fibre cement
be returned by the customer and reused several do not occur.
times.
Water
2.10 Condition of use No ingredients are washed out which could be
Hydration of the cement and water mixture forms hazardous to water (see also “Eluate analysis” in
hardened cement paste (calcium silicate hydrate) with Evidence). The pH value is alkaline (pH ≥ 10).
embedded fibres and fillers as well as micro air pores.
The fibre-cement products comprise approx. 6% water Mechanical destruction
(equilibrium moisture) and a proportion by volume of Not of relevance
approx. 30% air (contained in the micro-pores).
The hydrophobic finish is bound as a solid material 2.14 Re-use phase
during the use stage via penetration of the surface De-construction: Depending on the mounting system,
pores. The water evaporates. the structural panels can be removed non-destructively
After the binding agent has set and when used as by unscrewing or opening the studs.
designated, fibre cement products can be used for
practically any applications. No maintenance or repair Re-use / Further use: If undamaged, de-constructed
is required over the service life of the boards. panels can be re-used as backer board or as
foundation protection.
2.11 Environment and health during use
Environmental protection: According to the present Re-use / Further use: When separated by type, the
state of knowledge, hazards for water, air and soil uncoated and coated fibre-cement products referred to
cannot arise when the products under review are can be re-ground and re-used as additives in the
processed as designated (see chapter 7). manufacture of fibre cement (material recycling). When
sorted by type, the uncoated and coated fibre-cement
Health protection: When the construction products products in question are also suitable for further use as
are used as designated, no health hazards are known a filler and loose material in civil engineering,
in connection with the base materials used and the especially in road construction or for noise barriers
performance thereof in the condition of use (see (material recycling).
chapter 7).
2.15 Disposal
2.12 Reference service life Within the production process, most of the generated
The service life of Bluclad panels is comparable with waste is immediately re-used within the process.
the RSL of buildings. The service life according to the When after end-of-life re-using or recycling the boards
/BBSR/ is indicated to be >50 years. as described in the previous paragraph is not practical,
the boards can be disposed to landfill class II. The
There are no verifiable influences on ageing when the waste code in accordance with the /European Waste
products are applied in accordance with the generally Index/ is 170904.
accepted rules of technology.
2.13 Extraordinary effects 2.16 Further information
Further information and safety data sheets are
Fire available on the website: www.siniat.de.
Building materials class A2 as per /DIN 4102-1/, i.e.
limited combustibility.
4 Environmental Product Declaration ETEX – Bluclad Plaster Base Boards
3. LCA: Calculation rules
3.1 Declared Unit and electric power consumption as well as waste
This declaration refers to the production of 1m2 Bluclad management processes using best available life cycle
(10mm, grammage 12,9 kg/m2) manufactured in inventory (LCI) datasets. This includes input flows with
Kapelle-op-den-Bos, Belgium. a contribution of less than 1% of mass or energy.
Production of capital equipment, facilities and
Declared unit infrastructure required for manufacture are outside the
Name Value Unit scope of this assessment.
Declared unit 1 m²
Gross density * 1290 kg/m3 3.5 Background data
* within range of 1180 kg/m³ +-10% The /GaBi ts software/ was used to model the product
life cycle. The basic data in the GaBi database is
applied for energy, transportation, auxiliary products
3.2 System boundary and preliminary products. The software was revised in
Type of EPD: Cradle-to-gate with options. 2018.
The following life cycle stages and modules are Bluclad is produced in Belgium. Belgian datasets were
included: used for the grid mixes. For other processes for which
no Belgian datasets were available, European average
Production stage (A1-A3): datasets were used (EU-28).
 transportation and manufacturing of pre-
3.6 Data quality
products to the manufacturing site
The overall data quality and quality of the data
 energy consumption and use of auxiliary
collection can be described as good. All relevant flows
materials during production
were considered. Methodological choices are
 disposal of production wastes consistent throughout the model.
 production of packaging
3.7 Period under review
Etex provided production data based on an annual
Construction stage (A4-A5):
average of the year 2016.
 transportation of product to the construction
site 3.8 Allocation
 energy consumption during the installation of Production data refer to the declared product allocated
products from the overall production volume (m2 virtually
normalised to 5 mm thickness) in Kapelle-op-den-Bos,
 production of fixing and finishing material
Belgium.
 disposal of installation wastes including
Specific information on allocation within the
emissions of biogenic CO from cellulose
2 background data is given in the /GaBi documentation/
 disposal/incineration of packaging materials (http://www.gabi-
(potential benefits from energy substitution software.com/international/support/gabi/gabi-database-
within the incineration process are declared in 2018-lci-documentation/).
module D) including emissions of biogenic
3.9 Comparability
CO from renewable packaging materials
2 Basically, a comparison or an evaluation of EPD data
is only possible if all the data sets to be compared
Use stage (B1-B7): were created according to /EN 15804/ and the building
 efforts for the use of the product, context, respectively the product-specific
maintenance and operational efforts characteristics of performance, are taken into account.
GaBi ts serves as background database for the
End-of-life stage (C1-C4): calculation of the life cycle assessment /GaBi ts
 energy consumption for de-construction and software/.
demolition
 transportation to disposal
 waste processing and landfilling of product
3.3 Estimates and assumptions
No estimations or assumptions were made for the
production stage. Information on assumptions for the
scenarios in the life cycle of the product are described
in chapter 4.
3.4 Cut-off criteria
All available data from production processes were
considered, i.e., all pre-products used, thermal energy
4. LCA: Scenarios and additional technical information
5 Environmental Product Declaration ETEX – Bluclad Plaster Base Boards
Transport to the building site (A4)
Name Value Unit
Transport distance 600 km
Capacity utilisation (including
61 %
empty runs)
Installation into the building (A5)
Name Value Unit
Auxiliary Stainless steel screws 0.128 kg
Electricity consumption 0.02 kWh
Material loss 0,39 kg
Dust in the air * 0 kg
VOC in the air 0 kg
* See chapter 2.8 for details regarding prevention of
dust emissions.
Use or application of the installed product (B1) see
section 2.11 "Use"
No efforts and release of substances occur during the
normal (i.e. anticipated) use phase.
Maintenance (B2)
No efforts occur during maintenance.
Name Value Unit
Water consumption 0 m3
Auxiliary 0 kg
Other resources 0 kg
Electricity consumption 0 kWh
Other energy carriers 0 MJ
Waste materials resulting from
0 kg
maintenance
Operational energy use (B6) and Operational water
use (B7)
No efforts occur in modules B6 and B7.
Name Value Unit
Water consumption 0 m3
Electricity consumption 0 kWh
Other energy carriers 0 MJ
End of life (C1-C4)
Name Value Unit
Collected as mixed construction
13 kg
waste (panel incl. screws)
Recycling screws 0.1 kg
Landfilling 12.9 kg
6 Environmental Product Declaration ETEX – Bluclad Plaster Base Boards
5. LCA: Results
DESCRIPTION OF THE SYSTEM BOUNDARY (X = INCLUDED IN LCA; MND = MODULE NOT DECLARED)
BENEFITS AND
CONSTRUCTI LOADS
PRODUCT STAGE ON PROCESS USE STAGE END OF LIFE STAGE BEYOND THE
STAGE SYSTEM
BOUNDARIES
7 Environmental Product Declaration ETEX – Bluclad Plaster Base Boards
lairetam
waR
ylppus tropsnarT
gnirutcafunaM
eht
morf
tropsnarT
etis
eht
ot
etag
ylbmessA esU
ecnanetniaM
riapeR
tnemecalpeR tnemhsibrufeR
ygrene
lanoitarepO esu
retaw
lanoitarepO esu
noitcurtsnoc-eD
noitilomed tropsnarT
gnissecorp
etsaW
lasopsiD -esueR -yrevoceR -gnilcyceR laitnetop
A1 A2 A3 A4 A5 B1 B2 B3 B4 B5 B6 B7 C1 C2 C3 C4 D
X X X X X X X MNR MNR MNR X X X X X X X
RESULTS OF THE LCA - ENVIRONMENTAL IMPACT: 1 m² Bluclad
Param
Unit A1-A3 A4 A5 B1 B2 B6 B7 C1 C2 C3 C4 D
eter
GWP [kg CO2-Eq.] 6.50E+0 4.90E-1 7.38E-1 0.00E+0 0.00E+0 0.00E+0 0.00E+0 8.35E-3 4.10E-2 0.00E+0 1.67E+0 1.37E-1
ODP [kg CFC11-Eq.] 5.31E-12 1.33E-14 4.23E-13 0.00E+0 0.00E+0 0.00E+0 0.00E+0 3.71E-14 1.12E-15 0.00E+0 6.68E-14 1.62E-14
AP [kg SO2-Eq.] 1.70E-2 1.13E-3 3.42E-3 0.00E+0 0.00E+0 0.00E+0 0.00E+0 2.37E-5 9.49E-5 0.00E+0 1.49E-3 5.64E-4
EP [kg (PO4)3--Eq.] 2.56E-3 2.89E-4 3.10E-4 0.00E+0 0.00E+0 0.00E+0 0.00E+0 2.22E-6 2.42E-5 0.00E+0 2.33E-3 3.99E-5
POCP [kg ethene-Eq.] 3.17E-3 -3.84E-4 2.49E-4 0.00E+0 0.00E+0 0.00E+0 0.00E+0 1.49E-6 -3.22E-5 0.00E+0 4.55E-4 3.84E-5
ADPE [kg Sb-Eq.] 9.67E-6 4.00E-8 2.53E-5 0.00E+0 0.00E+0 0.00E+0 0.00E+0 4.44E-9 3.35E-9 0.00E+0 9.14E-8 3.15E-6
ADPF [MJ] 6.75E+1 6.63E+0 7.38E+0 0.00E+0 0.00E+0 0.00E+0 0.00E+0 8.89E-2 5.55E-1 0.00E+0 3.73E+0 1.52E+0
GWP = Global warming potential; ODP = Depletion potential of the stratospheric ozone layer; AP = Acidification potential of land and water; EP =
Caption Eutrophication potential; POCP = Formation potential of tropospheric ozone photochemical oxidants; ADPE = Abiotic depletion potential for non-
fossil resources; ADPF = Abiotic depletion potential for fossil resources
RESULTS OF THE LCA - RESOURCE USE: 1 m² Bluclad
Parameter Unit A1-A3 A4 A5 B1 B2 B6 B7 C1 C2 C3 C4 D
PERE [MJ] 1.97E+1 3.67E-1 1.84E+0 0.00E+0 0.00E+0 0.00E+0 0.00E+0 5.73E-2 3.07E-2 0.00E+0 4.11E-1 1.94E-1
PERM [MJ] 1.18E+1 0.00E+0 0.00E+0 0.00E+0 0.00E+0 0.00E+0 0.00E+0 0.00E+0 0.00E+0 0.00E+0 0.00E+0 0.00E+0
PERT [MJ] 3.15E+1 3.67E-1 1.84E+0 0.00E+0 0.00E+0 0.00E+0 0.00E+0 5.73E-2 3.07E-2 0.00E+0 4.11E-1 1.94E-1
PENRE [MJ] 7.82E+1 6.65E+0 8.21E+0 0.00E+0 0.00E+0 0.00E+0 0.00E+0 1.53E-1 5.57E-1 0.00E+0 3.87E+0 1.52E+0
PENRM [MJ] 0.00E+0 0.00E+0 0.00E+0 0.00E+0 0.00E+0 0.00E+0 0.00E+0 0.00E+0 0.00E+0 0.00E+0 0.00E+0 0.00E+0
PENRT [MJ] 7.82E+1 6.65E+0 8.21E+0 0.00E+0 0.00E+0 0.00E+0 0.00E+0 1.53E-1 5.57E-1 0.00E+0 3.87E+0 1.52E+0
SM [kg] 3.38E-1 0.00E+0 1.01E-2 0.00E+0 0.00E+0 0.00E+0 0.00E+0 0.00E+0 0.00E+0 0.00E+0 0.00E+0 0.00E+0
RSF [MJ] 0.00E+0 0.00E+0 0.00E+0 0.00E+0 0.00E+0 0.00E+0 0.00E+0 0.00E+0 0.00E+0 0.00E+0 0.00E+0 0.00E+0
NRSF [MJ] 0.00E+0 0.00E+0 0.00E+0 0.00E+0 0.00E+0 0.00E+0 0.00E+0 0.00E+0 0.00E+0 0.00E+0 0.00E+0 0.00E+0
FW [m³] 2.93E-2 6.76E-4 4.01E-3 0.00E+0 0.00E+0 0.00E+0 0.00E+0 7.81E-5 5.66E-5 0.00E+0 6.55E-4 1.64E-3
PERE = Use of renewable primary energy excluding renewable primary energy resources used as raw materials; PERM = Use of
renewable primary energy resources used as raw materials; PERT = Total use of renewable primary energy resources; PENRE = Use of
non-renewable primary energy excluding non-renewable primary energy resources used as raw materials; PENRM = Use of non-
Caption
renewable primary energy resources used as raw materials; PENRT = Total use of non-renewable primary energy resources; SM = Use
of secondary material; RSF = Use of renewable secondary fuels; NRSF = Use of non-renewable secondary fuels; FW = Use of net fresh
water
RESULTS OF THE LCA – OUTPUT FLOWS AND WASTE CATEGORIES:
1 m² Bluclad
Parameter Unit A1-A3 A4 A5 B1 B2 B6 B7 C1 C2 C3 C4 D
HWD [kg] 3.25E-7 3.85E-7 3.06E-8 0.00E+0 0.00E+0 0.00E+0 0.00E+0 7.16E-11 3.22E-8 0.00E+0 4.88E-8 9.84E-9
NHWD [kg] 5.35E-1 5.57E-4 4.54E-1 0.00E+0 0.00E+0 0.00E+0 0.00E+0 1.08E-4 4.67E-5 0.00E+0 1.27E+1 9.59E-3
RWD [kg] 4.22E-3 9.11E-6 3.28E-4 0.00E+0 0.00E+0 0.00E+0 0.00E+0 2.53E-5 7.63E-7 0.00E+0 5.56E-5 0.00E+0
CRU [kg] 0.00E+0 0.00E+0 0.00E+0 0.00E+0 0.00E+0 0.00E+0 0.00E+0 0.00E+0 0.00E+0 0.00E+0 0.00E+0 0.00E+0
MFR [kg] 0.00E+0 0.00E+0 2.24E-2 0.00E+0 0.00E+0 0.00E+0 0.00E+0 0.00E+0 0.00E+0 1.00E-1 0.00E+0 0.00E+0
MER [kg] 0.00E+0 0.00E+0 0.00E+0 0.00E+0 0.00E+0 0.00E+0 0.00E+0 0.00E+0 0.00E+0 0.00E+0 0.00E+0 0.00E+0
EEE [MJ] 0.00E+0 0.00E+0 0.00E+0 0.00E+0 0.00E+0 0.00E+0 0.00E+0 0.00E+0 0.00E+0 0.00E+0 0.00E+0 0.00E+0
EET [MJ] 0.00E+0 0.00E+0 0.00E+0 0.00E+0 0.00E+0 0.00E+0 0.00E+0 0.00E+0 0.00E+0 0.00E+0 0.00E+0 0.00E+0
HWD = Hazardous waste disposed; NHWD = Non-hazardous waste disposed; RWD = Radioactive waste disposed; CRU = Components
Caption for re-use; MFR = Materials for recycling; MER = Materials for energy recovery; EEE = Exported electrical energy; EEE = Exported
thermal energy
6. LCA: Interpretation
Considering the overall lifecycle, for most of the impact also strongly influenced by the landfilling of the
categories (except for ADPe and EP), the cellulose-containing materials.
manufacturing of Bluclad contributes to the largest
share (> 50 %) to the environmental performance. Within A1-A3 the pre-chains of the raw material have
the most important impact (contribution >50%)
For ADPe, the use of the stainless steel screws in A5 followed by the energy consumption for the production.
contributes most significantly to the results. The EP is The only exception is POCP which is mainly
determined by the energy consumption and direct Interpretation of LCA-results in A1:
production emissions (contribution >50%). Transport to The LCA for Bluclad is mainly determined by the pre-
the site (A2) has a negligible influence on the overall chains of the following raw materials: cement, cellulose
LCA results (contribution <2.5%). and silica sand flour. The contribution per impact
category varies within these raw materials. Cement is
The re-emission of organic CO2 inherent in packaging most important for GWP, POCP and ADPe. Whereas
materials (wooden pallets, cardboards) as well as in cellulose has a significant impact in AP and EP. The
cellulose takes place in module A5, in which the contribution of silica sand is lower in comparison to
packaging and the installation wastes are incinerated. cement and cellulose but shows a relevant impact for
ODP (contribution >25%). The Hydrofyer has some
influence only in the impact category ADPe.
7. Requisite evidence
7.1 Radioactivity 7.2 Leaching
Radioactivity measurements confirm that no other Leaching tests based on /EN 12457-2/ showed that no
gamma emitters than those originating from the natural hazardous compounds were leached out.
radiation sources are contained. The measured
radioactivity levels do not exceed the activity /Report on Leaching/
concentration indices as specified by the /Article 3
(Radiation Protection 112) for building products/ 7.3 VOC emissions
following the /Council Directive 96/29/. Bluclad boards are exclusively used in outdoor
applications. Evidence of volatile organic compound
Activity concentration index ≤ 2. (VOC) emissions is therefore not of relevance.
/Report on Radioactivity/
8. References
/Article 3 (Radiation Protection 112) for building DIN 4102-1:1998, Fire behaviour of building materials
products/ and elements - Classification of building materials -
Radiological Protection Principles concerning the Requirements and testing
Natural Radioactivity of Building Materials, published in
1999 by the Directorate-General Environment, Nuclear /DIN 53436/
Safety and Civil Protection DIN 53436-1:2015-12, Generation of thermal
decomposition products from materials for their
/BAM/ analytic-toxicological testing - Part 1: Decomposition
Material Testing Institute of the state of apparatus and determination of test temperature
Brandenburg/Berlin and the German Federal Institute
for Materials Research and Testing /EN 12457-2/
NF EN 12457-2 December 2002, Characterization of
/BBSR/ waste - Leaching - Compliance test for leaching of
BBSR table "Service lives of components for life cycle granular waste materials and sludges - Part 2 : one
assessment according to Bewertungssystem stage batch test at a liquid to solid ratio of 10 l/kg for
Nachhaltiges Bauen (BNB)" Sustainable Building materials with particle size below 4 mm (without or with
Information Portal by the Federal Ministry of Transport, size reduction)
Building and Urban Affairs (Bundesinstitut für Bau-,
Stadt- und Raumforschung, BBSR) /EN 12467/
https://www.nachhaltigesbauen.de/baustoff-und- NF EN 12467, November 2012, Fibre-cement flat
gebaeudedaten/nutzungsdauern-von-bauteilen.html sheets - Product specification and test methods
/Construction Products Regulation/ /EN 13501-1/
Regulation (EU) No 305/2011 of the European NF EN 13501-1+A1, February 2013, Fire classification
Parliament and of the Council of 9 March 2011 laying of construction products and building elements - Part
down harmonised conditions for the marketing of 1: classification using data from reaction to fire tests
construction products and repealing Council Directive
89/106/EEC Text with EEA relevance /EN 197-1/
DIN EN 197-1:2011-11, Cement - Part 1: Composition,
/Council Directive 96/29/ specifications and conformity criteria for common
Council Directive 96/29/Euratom of 13 May 1996 cement; German version EN 197-1:2011
laying down basic safety standards for the protection of
9 Environmental Product Declaration Promat – /Eurofins Analyses pour l’Environnement/
PROMATECT-H Eurofins Analyses pour l'Environnement France
the health of workers and the general public against 5, rue d'Otterswiller
the dangers arising from ionizing radiation 67700, Saverne
France
/DIN 4102-1/
/Eurofins Product Testing A/S/
Smedeskovvej 38
8 Environmental Product Declaration ETEX – Bluclad Plaster Base Boards
DK - 8464
Galten /REACH Regulation/
Denmark Regulation (EU) No 1907/2006 of the
European Parliament and of the Council of 18
European Waste Index/ December 2006 concerning the Registration,
European Waste Index provides an EU-wide common Evaluation, Authorisation and Restriction of Chemicals
terminology for waste classification. The index is in the (REACH), establishing an European Chemicals
Commission Decision of 3 May 2000 Agency, amending Directive 1999/45/EC and repealing
Council Regulation (EEC) No 793/93 and Commission
/GaBi documentation/ Regulation (EC) No 1488/94 as well as Council
GaBi 8.7 data set documentation for the software Directive 76/769/EEC and Commission Directives
system and data bases, LBP, University of Stuttgart 91/155/EEC, 93/67/EEC, 93/105/EC and 2000/21/EC
and thinkstep AG, Leinfelden-Echterdingen, 2018,
http://www.gabi- /Report on Radioactivity/
software.com/international/support/gabi/gabi-database- Date: 2 December 2011
2018-lci-documentation/ Measuring agency: /SCK.CEN Laboratory for Gamma
spectrometry/, Mol, Belgium
/GaBi ts software/ Protocol: Activity concentration index (ACI)
GaBi Software-System and Database for Life Cycle
Engineering, 1992-2018, thinkstep AG, Leinfelden- /Report on Leaching/
Echterdingen, with acknowledgement of LBP Date: 26 June 2015
University of Stuttgart, program version 8.7 Measuring agency: /Eurofins Analyses pour
l’Environnement/ France-Site de Saverne
/ISO 14001/
UNI EN ISO 14001:2015, Environmental management /SCK.CEN Laboratory for Gamma spectrometry/
systems - Requirements with guidance for use SCK•CEN Research Center MolBoeretang 200
2400 Mol
/ISO 9001/ België
UNI EN ISO 9001:2015, September 2015, Quality
management systems - Requirements /Z-31.4-160/
General technical approval no. Z-31.4-160 of the
/OHSAS 18001/ "Deutsches Institut für Bautechnik" (DIBt) for Eternit
OHSAS 18001:2007, Occupational Health and Safety facade panels
Management Certification
/IBU 2016/
/Ordinance on Biocide Products/ IBU (2016): General Programme Instructions for the
Regulation (EU) No 528/2012 of the Preparation of EPDs at the Institut Bauen und Umwelt
European Parliament and of the Council of 22 May e.V., Version 1.1 Institut Bauen und Umwelt e.V.,
2012 concerning the making available on the market Berlin.
and use of biocidal products www.ibu-epd.de
/PCR Part A/ /ISO 14025/
PCR Part A: Calculation rules for the LCA and DIN EN /ISO 14025:2011-10/, Environmental labels
requirements on the Background Report, Version 1.7, and declarations — Type III environmental
Institut Bauen und Umwelt e.V., www.epd-online.com, declarations — Principles and procedures
2018
/EN 15804/
/PCR Part B/ /EN 15804:2012-04+A1 2013/, Sustainability of
PCR Part B: Requirements on the EPD for Fibre construction works — Environmental Product
cement / Fibre concrete, Version 1.6, Institut Bauen Declarations — Core rules for the product category of
und Umwelt e.V., www.bau-umwelt.com, 2017 construction products
9 Environmental Product Declaration ETEX – Bluclad Plaster Base Boards
Publisher
Institut Bauen und Umwelt e.V. Tel +49 (0)30 3087748- 0
Panoramastr. 1 Fax +49 (0)30 3087748- 29
10178 Berlin Mail info@ibu-epd.com
Germany Web www.ibu-epd.com
Programme holder
Institut Bauen und Umwelt e.V. Tel +49 (0)30 - 3087748- 0
Panoramastr 1 Fax +49 (0)30 – 3087748 - 29
10178 Berlin Mail info@ibu-epd.com
Germany Web www.ibu-epd.com
Author of the Life Cycle
Assessment Tel +49 711 341817-0
thinkstep AG Fax +49 711 341817-25
Hauptstraße 111- 113 Mail info@thinkstep.com
70771 Leinfelden-Echterdingen Web http://www.thinkstep.com
Germany
Owner of the Declaration
Etex Building Performance Tel +32 2 778 12 11
International Fax +32 2 778 12 12
Marcel Demonque 500 r Mail info@etexgroup.com
84915 Avignon Cedex 9 Web http://www.etexgroup.com
France
