ENVIRONMENTAL PRODUCT DECLARATION
as per ISO 14025 and EN 15804+A1
Owner of the Declaration NMC S.A.
Programme holder Institut Bauen und Umwelt e.V. (IBU)
Publisher Institut Bauen und Umwelt e.V. (IBU)
Declaration number EPD-NMC-20210312-IBD1-EN
Issue date 05.01.2022
Valid to 04.01.2027
CLIMAFLEX®naturefoam easy
NMC S.A.
www.ibu-epd.com | https://epd-online.com
Umwelt Produktdeklaration Name des Herstellers – Name des Produkts
1. General Information
NMC S.A. CLIMAFLEX®naturefoam easy
Programme holder Owner of the declaration
IBU – Institut Bauen und Umwelt e.V. NMC S.A.
Panoramastr. 1 Gert-Noel Strasse
10178 Berlin BE-4731 Eynatten
Germany
Declaration number Declared product / declared unit
EPD-NMC-20210312-IBD1-EN 1 m³ insulation material CLIMAFLEX®naturefoam easy
This declaration is based on the product Scope:
category rules: Product line CLIMAFLEX®naturefoam easy
Insulating materials made of foam plastics, 01.2019 Thermal insulation products for building equipment and
(PCR checked and approved by the SVR) industrial insulations made of polythene foam (PEF)
according to EN14313. This declaration is an
Environmental Product Declaration according to
Issue date
/ISO14025/ describing the specific environmental
05.01.2022
performance of the product produced in Belgium at the
side of Eynatten.
Valid to
04.01.2027
The owner of the declaration shall be liable for the
underlying information and evidence; the IBU shall not
be liable with respect to manufacturer information, life
cycle assessment data and evidences.
The EPD was created according to the specifications
of EN 15804+A1. In the following, the standard will be
simplified as EN 15804.
Verification
The standard EN 15804 serves as the core PCR
Independent verification of the declaration and data
according to ISO 14025:2010
Dipl. Ing. Hans Peters internally x externally
(chairman of Institut Bauen und Umwelt e.V.)
Dr. Alexander Röder Vito D'Incognito
(Managing Director Institut Bauen und Umwelt e.V.)) (Independent verifier)
2. Product
2.1 Product description/Product definition installations for a reference service life (RSL) of 50
CLIMAFLEX®naturefoam easy Polyethylene foams years.
have many environmental benefits, having a low This duration is based on the frequency of replacement
density (average 28 kg/m³), few raw materials are of sanitary and heating piping in buildings. Although
required for the manufacture of an article and the the insulation pipes are still effective after 50 years, it
environmental impact of their transport is lower than is assumed that when replacing the piping, the
similar articles of higher density performing the same insulation CLIMAFLEX®naturefoam easy is not reused
function. and is recycled. 50 years is the minimum Reference
The CLIMAFLEX®naturefoam easy does have a self Service Life recommended for factory made thermal
adhesive strip. Furthermore, insulation products”.
the CLIMAFLEX®naturefoam easy are recyclable with
exception of the self-adhesive strip. 2.3 Technical Data
Performance data of the product in accordance with
For the placing on the market of the product in the the Declaration of Performance with respect to its
European Union/European Free Trade Association Essential Characteristics according to /EN 14313/
(EU/EFTA) (with the exception of Switzerland) - apply. Further data:
Thermal Insulation products for building equipment and
industrial installations. Factory made polyethylene
foam (PEF) and the CE-marking. For the application Constructional data
and use the respective national provisions apply. Performance data of the product in accordance with
2.2 Application the Declaration of Performance with respect to its
The function of CLIMAFLEX®naturefoam easy is to Essential Characteristics according to /EN 14313/
ensure the insulation of heating and sanitary apply. Further data:
2 Environmental Product Declaration NMC sa – CLIMAFLEX®naturefoam easy
Name Value Unit
Gross density 28 kg/m3 Name Value Unit
Thermal conductivity At 40 °C 0.04 W/(mK) Bio LDPE 58,79 %
Reaction to Fire Acc.to /EN Bl-s1d0 ; Polyethylene 1.23 %
-
13501-1/ Cl-s1d0 NMC Internally recycled PE 16.8 %
Max Service Temperature Acc. to Flame retardant 4.15 %
100 °C
/EN 14707 Pigments and fillers 2.0 %
Min Service Temperature 0 °C Volume stabilizer 1,37 %
Water absorption Acc. to EN Blowing Agent 9.11 %
WS005
13472 Double-sided self-adhesive 5.18 %
Traces quantities of water soluble Cl < 15 – F Release band 1.37 %
ions and pH-value Acc. to EN < 4 - pH
13468 and EN 13472 6,1 BIO-PE and fillers are the main components of the
product and are responsible for the characteristics and
performance of the product
The blowing agent causes the expansion during
manufacturing. The flame retardant ensures the fire
2.4 Delivery status resistance and conformity with fire protection
The CLIMAFLEX®naturefoam easy product is a regulations (see section 2.13).
closed-cell bio-polyethylene foam insulation tube According to the European Chemicals Regulation
designed for applications in heating and sanitary “REACH” manufacturers, importers and downstream
installations. The EPD will cover the whole users must register their chemicals and are
CLIMAFLEX®naturefoam easy range. The insulating responsible for their safe use. NMC S.A. uses
sleeves in the CLIMAFLEX®naturefoam easy range exclusively verifiably registered and approved
have a thickness ranging from 9 to 20mm and an substances in its production. Products manufactured
inside diameter ranging from 15 to 102mm .These and put on the market by NMC do need to be
products are categorized according to thickness. The registered. CLIMAFLEX®naturefoam easy do not
category of small thickness products includes the contain Substances of Very High Concern (SVHC).
CLIMAFLEX® naturefoam easy 9 and 13mm products Antimony trioxide and halogenated flame retardants
while the category of large thickness products includes are applied.
CLIMAFLEX®naturefoam easy 20 and 25mm
products. These two categories are also distinguished
by their rating in fire reaction tests. For small thickness
products (9 and 13mm) the fire classification is
2.6 Manufacture
Euroclass Bl s1 d0 (Acc. to EN 13501-1) and for large
The manufacture of the CLIMAFLEX®naturefoam easy
thickness products (20mm) the fire rating is Euroclass
product consists of incorporating the ingredients of the
Cl s1 d0 (Acc. to EN 13501-1).
formulation into an extruder, adding a foaming agent,
mixing, heating and then extruding the mix through a
die, during which time foaming takes place. The
2.5 Base materials/Ancillary materials
product is then cooled with water (municipal water),
drying and the double-sided self-adhesive is applied as
Base materials
well as the release band. After that the product is cut to
CLIMAFLEX®naturefoam easy is a professional bio-
size before being packed and stored.
polyethylene-based closed-cell foam pipe insulation for
continuous energy saving and condensation control
Quality assurance :
purposes. CLIMAFLEX®naturefoam easy provides
The manufacture is certified ISO 9001 for the quality
solutions that follow all necessary guidelines and
management and the product is certified for CE
standards for any type of installation. The
marking according to CPR (CE Certificate of
CLIMAFLEX®naturefoam easy is equipped with a
conformity N° 0749-CPR-BC1-571-4133-0001-01and
double-sided self-adhesive means that installed pipes
0749-CPR-BC1-571-4133-0002-01)
can be insulated twice as quickly as with traditional
insulation products. The following table displays the
different elements of the formulation for
2.7 Environment and health during
CLIMAFLEX®naturefoam easy. This is in accordance
manufacturing
with the PCR Part B: Requirements on the EPD for
During all manufacturing steps of NMC S.A. Belgium,
Insulating materials made of foam plastics and ISO
the production follows all national guidelines and
14025.
regulations. Solar panels are installed on the roof of
the warehouse and in the field to reduce the
This product contains substances listed in the requirement for grid electricity.
candidate list (date: 08.07.2021) exceeding 0.1
percentage by mass: No. 2.8 Product processing/Installation
This product contains other CMR substances in CLIMAFLEX®naturefoam easy can be installed using
categories 1A or 1B, which are not on the candidate basic tools (e.g. craft knives) and thus have a self
list, exceeding 0.1 percentage by mass: No. adhesive strip for easy application on installed pipes.
No special tools, nor specific protection is necessary.
Biocide products were added to this construction When applying adhesives the information given in the
product or it has been treated with biocide products relevant safety data sheets is to be heeded.
(this then concerns a treated product as defined by the Any glue and adhesive tapes used during the
(EU) Ordinance on Biocide Products No. installation phase were not included in the
528/2012): No. LCA. Recommendations on how to use the product are
3 Environmental Product Declaration NMC sa – CLIMAFLEX®naturefoam easy
described in the application manuals or videos. More
details are listed on the Web Page www.nmc-
insulation.com 2.13 Extraordinary effects
2.9 Packaging Fire
CLIMAFLEX®naturefoam easy products are packed in CLIMAFLEX®naturefoam easy is classified as a
cardboard boxes and transported on reusable pallets. combustible insulation material. Due to its material
All packaging material can be recycled. The pallets structure, CLIMAFLEX®naturefoam easy does not
used to transport the products are taken back or contribute to an uncontrollable spread of fire under
exchanged when the CLIMAFLEX®naturefoam easy is installation conditions typical on a building site. The
delivered, so the use of pallets is a close loop product is self-extinguishing reducing its contribution to
economy. any fire event. There is no possibility of the material
self-igniting. CLIMAFLEX®naturefoam easy does not
propagate the fire horizontally or vertically. The smoke
development in case of fire is very low (class S1).
2.10 Condition of use
During the use of the products for the purpose for
which they are intended, there are no modifications
unless one of the effects listed in extraordinary impacts Fire protection
occurs (see point 2.13). Name Value
Building material class Bl / Cl
2.11 Environment and health during use Burning droplets d0
There are no particular effects on environmental and Smoke gas development S1
health impacts during use related to the material
composition of the product. The Water
CLIMAFLEX®naturefoam easy products are used in a CLIMAFLEX®naturefoam easy is a closed cell foam
wide range of applications across the building sector. and obtains the best water absorption class WS005
The PEF foams fulfil the German, Belgian and French according to the product standard
regulations regarding the emission of VOC with
emissions far below the most stringent limit values.
The Eurofin Product Testing institute, at the request of Mechanical destruction
the CEFEP (European group of PEF and FEF CLIMAFLEX®naturefoam easy is chemically inert and
manufacturers) has made a wide range of tests for does not present any environmental or health risk if
different PEF products from different manufacturers. mechanically destructed. CLIMAFLEX®naturefoam
easy is not UV resistant. The product is not
The insulation of heating pipes with recommended for outside applications without
CLIMAFLEX®naturefoam easy allows a reduction complementary UV protection
energy dispertion and of course CO emissions during
2
the full service life of the installation. The quantification 2.14 Re-use phase
of this in-use benefit is not within the scope of this In principle, if removed carefully,
EPD, however, this could be calculated using an LCA CLIMAFLEX®naturefoam easy can be reused on any
for the complete pipe/insulation system, and has to be other piping system of similar dimensions. Any material
evaluated in the frame of the LCA from the complete not suitable for reuse is fully recyclable.
heating installation. A software program available on
NMC’s website http://cit.nmc-insulation.com/ allows for 2.15 Disposal
the calculation of the heat flow and insulation benefit The CLIMAFLEX®naturefoam easy is recyclable with
under real use conditions. exception of the self-adhesive strip and can be used as
a substitute for virgin PE-LD granulates, with only
2.12 Reference service life minor additive additions. There is no chemical
The function of CLIMAFLEX®naturefoam easy is to difference between bio-based PE-LD and fossil fuel
insure the insulation of heating and sanitary derived PE-LD, so using a mix of sources does not
installations for a reference service life (RSL) of 50 change the recyclability of the product.
years. This duration is based on the frequency of
replacement of sanitary and heating piping in buildings. 2.16 Further information
Although the insulation pipes are still effective after 50 Additional information about CLIMAFLEX®naturefoam
years, it is assumed that when replacing the piping, the easy can be found on the NMC web site www.nmc-
insulation (CLIMAFLEX®naturefoam easy) is recycled. insulation.com Here specification clauses, data sheets
50 years is the minimum Reference Service Life and application manuals can be found.
recommended in /EN16783/ “PCR for factory made
thermal insulation products”.
3. LCA: Calculation rules
3.1 Declared Unit average reference density of CLIMAFLEX®naturefoam
The declared unit for insulating materials made of foam easy is 28 kg/m³.
plastic is 1 m³. The EPD will cover the
whole CLIMAFLEX®naturefoam easy range. The
insulating sleeves in the CLIMAFLEX®naturefoam Declared unit
easy range have a thickness ranging from 9 to 20 mm Name Value Unit
thick and from 15 to 102mm inside diameter The Declared unit 1 m3
4 Environmental Product Declaration NMC sa – CLIMAFLEX®naturefoam easy
Gross density 28 kg/m3 Module C1: As for the installation of the product, the
Volume for 1kg 0.0357 m³ disassembly is done manually and does not require
Value for 1 any specific equipment. Disassembly is generally
m3 carried out at the same time as the replacement or
divided removal of sanitary pipes. Consequently, there are no
Conversion Factor from 1 m3 to 1
section of m impacts associated with C1.
linear meter
the Module C2: Transport at end-of-life stage is modeled
insulation as a Euro Cargo 0-6 mix truck with diesel fuel. The
pipe ( m²) average distance to either mechanical recycling,
Thermal Conductivity λ : 0.040 W/mK at (40°C) incineration or landfills is assumed to be 100 km
R-value- thickness- : 25 mm : +/- 3.5 (m²K/W)
depending on the pipe diameter. Module C3:The scenario that has been retained for
this Life Cycle Assessment is the 100% recycling
scenario.
3.2 System boundary Module C4: As CLIMAFLEX®naturefoam easy is fully
The Data collection refers to the yearly production in recyclable, the legislation is pushing more in this
2020. direction and the overall pressure on plastic recycling
is growing, the scenario with recycling is considered.
Module A1 to A3: The LCA calculation covers the
production of the raw materials, transport of these to Module D:The CLIMAFLEX®naturefoam easy is
the plant, the mixing of raw materials according to the recyclable with exeption of the self adhesive strip and
respective recipes, manufacturing of the foam product can be used as a substitute for virgin PE-LD
and packaging for dispatch. All production takes place granulates, with only minor additive additions. There is
exclusively in Eynatten, Belgium. no chemical difference between bio-based PE-LD and
fossil fuel derived PE-LD, so using a mix of sources
Module A4: NMC’s logistics department reported does not change the recyclability of the product.
average figures for the distribution of NMC’s products -
depending on the country the transport distance 3.3 Estimates and assumptions
varies. In the table below shows, the biggest The LCA calculation is conducted using the Gabi ts -
customers sorted by country as well as the volumes of database. Not all necessary LCIs are included in the
CLIMAFLEX®naturefoam easy delivered. These database. Where data were missing or were
customers represent 85,2% of sales volumes in 2020, unavailable or where suppliers were unable to provide
with the remainder supplied to a large set of smaller complete information, proxy datasets have been used.
customers. The environmental burden for the production of
pigments, flame retardants and volume stabilizers are
Module A5: Installation of CLIMAFLEX®naturefoam approximated.
easy products is done by hand and requires no special
equipment apart from a knife. The products can be
placed end to end and the remaining pieces can be 3.4 Cut-off criteria
reused. Some glue or tape could be used for the Any glue and adhesive tapes, on behalf of the self
installation, as the quantity or the product used adhesive-strip of the product, used during the
depends on the final customer, he has to calculate the installation (A5) have not been included as
impact of what he used himself. The environmental quantification of these materials is uncertain and their
impact of this type of accessory is not counted in this use by the various installers is too diverse, adhesives
study. The calculations do not contain any installation and glues are not required in all/most cases, but may
waste. Cardboard as packaging material is assumed to be used for some applications.
be recycled. As input material cardboard made of In this study no others cut-off criteria have been
waste paper is considered. Thus, environmental applied and all elementary incoming processes as well
burden for packaging materials are considered already as all energy and water inputs and waste outputs have
in A1-A3. The value of the environmental impact for A5 been counted.
is declared as “0”. The choice made is : the final user
have to calculate the impact of A5 himself in function of 3.5 Background data
his own case, by accounting for the extra amount of The software system for life cycle engineering /GaBi
product needed during installation. 10/ developed by thinkstep AG was used to perform
this LCA. The GaBi LCI database /GaBi 10/ provides
Module B1-B7:Once installed the the life cycle inventory data for several of the raw and
CLIMAFLEX®naturefoam easy product requires no process materials obtained from the background
maintenance and no repair. It will be dismantled when system. The most recent update of the database was
the sanitary pipe is replaced. For this reason, there are in 2020.
not expected to be any impacts in B1 to B7 assuming
correct specification and installation. The step B1 is not 3.6 Data quality
considered in this LCA, although the insulation of the All the foreground data requiring such energy or raw
piping contributes to a significant reduction of CO material coming from production, were verified and
2
emissions from the heating or cooling equipment, this cross-checked before being included in the model.
is not taken into account in this LCA. It should, Most of the life cycle inventories for the basic materials
however, be taken into account in the calculation of are available in the/ GaBi 10/ database.
environmental impacts of the complete heating and For electrical and thermal energy Belgium specific grid
cooling systems or of the complete building. mixes and Belgium specific supply for natural gas were
considered.
5 Environmental Product Declaration NMC sa – CLIMAFLEX®naturefoam easy
3.7 Period under review
The production data for the year 2020 were used for
the realization of this study. 3.9 Comparability
Basically, a comparison or an evaluation of EPD data
3.8 Allocation is only possible if all the data sets to be compared
There is no co-product or by-product generated during were created according to EN 15804 and the building
the production of NMC’s products. context, respectively the product-specific
Due to the lack of specific data per production line and characteristics of performance, are taken into account.
product, the energy has been allocated per overall
produced volume of insulation foam.
Production waste
Most of the production waste from the process
(machine start, end of production, non-conforming
products, etc.) is recycled internally in order to be
reused in the manufacturing process. These impacts
are accounted for in A1-A3.
Installation and End-of-Life waste
Installation of the foam products is done by hand and
requires no special equipment apart from a knife.
Installation off-cut is not considered in this calculations.
Any glue and adhesive tapes used during the
installation phase were not included in the LCA.
4. LCA: Scenarios and additional technical information
Material loss - kg
Transport to the building site (A4) Replacement (B4) / Refurbishment (B5)
Name Value Unit Name Value Unit
Litres of fuel 0.118 l/100km Number/
Replacement cycle -
Transport distance 332 km RSL
Capacity utilisation (including Electricity consumption - kWh
10 %
empty runs) Litres of fuel - l/100km
Gross density of products Replacement of worn parts - kg
28 kg/m3
transported
Installation into the building (A5) Reference service life
Name Value Unit Name Value Unit
Reference service life years 50 a
Use or application of the installed product (B1) see
section 2.12 "Use" Operational energy use (B6) and Operational water
Name Value Unit use (B7)
Name Value Unit
Maintenance (B2) Water consumption - m3
Name Value Unit Electricity consumption - kWh
Information on maintenance - -
Other energy carriers - MJ
Number/
Maintenance cycle - Equipment output - kW
RSL
Water consumption - m3
End of life (C1-C4)
Auxiliary - kg
Name Value Unit
Other resources - kg Recycling 29.8 kg
Electricity consumption - kWh
Other energy carriers - MJ Reuse, recovery and/or recycling potentials (D),
Material loss - kg relevant scenario information
One of the benefits beyond the boundaries of the
Repair (B3) system is the recyclability of the Climaflex product.
Name Value Unit Recycled PE-LD granulate can be used as a substitute
Information on the repair process - - for virgin PE-LD granulate on a one-for-one basis.
Information on the inspection process - - Furthermore, there are no differences in the properties
Number/ or performance of bio-based PE-LD and PE-LD
Repair cycle -
RSL derived from fossil fuels. It is assumed that recycled
Water consumption - m3 granulate generated from Climaflex products displace
Auxiliary - kg the need for fossil fuel derived PE-LD granulate.
Other resources - kg
Electricity consumption - kWh Another benefit beyond the boundaries of the system
Other energy carriers - MJ is the recovery of energy generated from the
6 Environmental Product Declaration NMC sa – CLIMAFLEX®naturefoam easy
incineration of waste at end-of-life. This is modeled in
the GaBi7 software using an industry-average dataset
for the incineration of polyethylene and according to
the quantity of waste at end-of-life. The recovery of
thermal and electrical energy produced by the
incinerator avoids the use of fossil resources.
Name Value Unit
7 Environmental Product Declaration NMC sa – CLIMAFLEX®naturefoam easy
5. LCA: Results
DESCRIPTION OF THE SYSTEM BOUNDARY (X = INCLUDED IN LCA; MND = MODULE NOT DECLARED;
MNR = MODULE NOT RELEVANT)
BENEFITS AND
CONSTRUCTI LOADS
PRODUCT STAGE ON PROCESS USE STAGE END OF LIFE STAGE BEYOND THE
STAGE SYSTEM
BOUNDARIES
8 Environmental Product Declaration NMC sa – CLIMAFLEX®naturefoam easy
lairetam
waR
ylppus tropsnarT
gnirutcafunaM
eht
morf
tropsnarT
etis
eht
ot
etag
ylbmessA esU
ecnanetniaM
riapeR
tnemecalpeR tnemhsibrufeR
ygrene
lanoitarepO esu
retaw
lanoitarepO esu
noitcurtsnoc-eD
noitilomed tropsnarT
gnissecorp
etsaW
lasopsiD -esueR -yrevoceR -gnilcyceR laitnetop
A1 A2 A3 A4 A5 B1 B2 B3 B4 B5 B6 B7 C1 C2 C3 C4 D
X X X X X MND MND MNR MNR MNR MND MND MND X X X X
RESULTS OF THE LCA - ENVIRONMENTAL IMPACT according to EN 15804+A1: 1 m³ CLIMAFLEX®
naturefoam easy
Parameter Unit A1-A3 A4 A5 C2 C3 C4 D
GWP [kg CO2-Eq.] 14.78 2.58 0.00 0.18 1.93 0.00 -54.42
ODP [kg CFC11-Eq.] 5.68E-8 2.43E-16 0.00E+0 4.75E-17 1.73E-13 0.00E+0 -7.22E-13
AP [kg SO2-Eq.] 7.16E-1 5.64E-2 0.00E+0 1.52E-4 1.99E-3 0.00E+0 -6.19E-2
EP [kg (PO4)3--Eq.] 6.54E-1 6.06E-3 0.00E+0 3.05E-5 4.84E-4 0.00E+0 -9.75E-3
POCP [kg ethene-Eq.] 1.90E-1 3.02E-3 0.00E+0 1.98E-5 2.31E-4 0.00E+0 -1.10E-2
ADPE [kg Sb-Eq.] 1.45E-1 1.25E-7 0.00E+0 1.60E-8 1.43E-6 0.00E+0 -1.32E-5
ADPF [MJ] 1080.90 34.47 0.00 2.38 25.58 0.00 -2106.53
GWP = Global warming potential; ODP = Depletion potential of the stratospheric ozone layer; AP = Acidification potential of land and water; EP =
Caption Eutrophication potential; POCP = Formation potential of tropospheric ozone photochemical oxidants; ADPE = Abiotic depletion potential for non-
fossil resources; ADPF = Abiotic depletion potential for fossil resources
RESULTS OF THE LCA - INDICATORS TO DESCRIBE RESOURCE USE according to EN 15804+A1: 1 m³
CLIMAFLEX® naturefoam easy
Parameter Unit A1-A3 A4 A5 C2 C3 C4 D
PERE [MJ] 1610.09 0.73 0.00 0.14 25.89 0.00 -132.50
PERM [MJ] 838.16 0.00 0.00 0.00 0.00 0.00 0.00
PERT [MJ] 2448.25 0.73 0.00 0.14 25.89 0.00 -132.50
PENRE [MJ] 1225.79 34.64 0.00 2.41 77.50 0.00 -2150.48
PENRM [MJ] 131.83 0.00 0.00 0.00 0.00 0.00 0.00
PENRT [MJ] 1357.62 34.64 0.00 2.41 77.50 0.00 -2150.48
SM [kg] 11.73 0.00 0.00 0.00 0.00 0.00 0.00
RSF [MJ] 0.00 0.00 0.00 0.00 0.00 0.00 0.00
NRSF [MJ] 0.00 0.00 0.00 0.00 0.00 0.00 0.00
FW [m³] 0.19 0.00 0.00 0.00 0.02 0.00 -0.24
PERE = Use of renewable primary energy excluding renewable primary energy resources used as raw materials; PERM = Use of
renewable primary energy resources used as raw materials; PERT = Total use of renewable primary energy resources; PENRE = Use of
non-renewable primary energy excluding non-renewable primary energy resources used as raw materials; PENRM = Use of non-
Caption
renewable primary energy resources used as raw materials; PENRT = Total use of non-renewable primary energy resources; SM = Use
of secondary material; RSF = Use of renewable secondary fuels; NRSF = Use of non-renewable secondary fuels; FW = Use of net fresh
water
RESULTS OF THE LCA – WASTE CATEGORIES AND OUTPUT FLOWS according to EN 15804+A1:
1 m³ CLIMAFLEX® naturefoam easy
Parameter Unit A1-A3 A4 A5 C2 C3 C4 D
HWD [kg] 4.83E-4 6.52E-10 0.00E+0 1.27E-10 2.65E-8 0.00E+0 -3.16E-7
NHWD [kg] 8.13E+0 1.88E-3 0.00E+0 3.79E-4 8.47E-2 0.00E+0 -5.87E-1
RWD [kg] 8.43E-2 2.28E-5 0.00E+0 4.38E-6 2.04E-2 0.00E+0 -1.65E-2
CRU [kg] 0.00 0.00 0.00 0.00 0.00 0.00 0.00
MFR [kg] 0.00 0.00 11.73 0.00 29.84 0.00 0.00
MER [kg] 0.00 0.00 0.00 0.00 0.00 0.00 0.00
EEE [MJ] 0.00 0.00 0.00 0.00 0.00 0.00 0.00
EET [MJ] 0.00 0.00 0.00 0.00 0.00 0.00 0.00
HWD = Hazardous waste disposed; NHWD = Non-hazardous waste disposed; RWD = Radioactive waste disposed; CRU = Components
Caption for re-use; MFR = Materials for recycling; MER = Materials for energy recovery; EEE = Exported electrical energy; EET = Exported
thermal energy
6. LCA: Interpretation
The base polymer used at NMC is produced from of the advantages of using a biopolymer is a significant
renewable raw materials (Biomass/Sugar cane). One reduction in greenhouse gas emissions compared to
the use of raw materials of fossil origin. In addition, the their transport account for most of 80% of the impact
use of non-renewable raw materials is avoided in this Global Warming Potential.
way. As the CLIMAFLEX®naturefoam easy is fully
When we analyse the complete life cycle we see that recyclable; the choice for the end of life was that of
the most impacting part for all environmental impact 100% recycling. This avoids the use of new raw
factors is the production module and more particularly materials and or the exploitation of renewable or non-
the raw materials part. With regard to global warming renewable resources.
for the complete life cycle, more than 78% comes from One way to continue to reduce the environmental
the production module 10,8 % of transport to the impact of the CLIMAFLEX® naturefoam easy would be
places of installation and 11,4% comes from the end of to continue to diversify our energy sources by
life. For all other impact factors, more than 90% of the switching more and more to renewable energies. To
impacts come from the production phase. this end, after having greatly increased the number of
Transport has a more pronounced impact on global photovoltaic panels, NMC will acquire a cogeneration
warming potential as well as on soil and water system. Looking for more eco-responsible suppliers
acidification potential and abiotic fossil resource must also be put in place, as well as finding raw
depletion potential materials manufactured locally to avoid long-distance
A more in-depth analysis of the production module A1 transport as much as possible.
to A3 shows that the production of raw materials and
7. Requisite evidence
7.1. VOC emissions Sum SVOC (C16 - C22) - μg/m3
Eurofins Product Testing A/S has tested a wide range R (dimensionless) - -
and variety of typical PEF (Polyethylene foam) VOC without NIK - μg/m3
products marketed in the EU from CEFEP (European Carcinogenic Substances - μg/m3
Group of PEF/FEF manufacturers) Based on the
loading factor 0.05m²/m3 (determined after AgBB overview of results (3 days [µg/m³])
consideration of the real life applications of PEF Name Value Unit
products (in living rooms) and recommendations by the TVOC (C6 - C16) - μg/m3
experts of the test institute) all results were found to be Sum SVOC (C16 - C22) - μg/m3
clearly below the limit values. For all samples below
R (dimensionless) - -
100mg/m3 TVOC after 28 days. Certificates are
VOC without NIK - μg/m3
available on request.
Carcinogenic Substances - μg/m3
7.2 Leaching
VOC Emissions
According to /EN 13468/ the content of water-soluble
Name Value Unit
chloride ions for CLIMAFLEX®naturefoam easy is
Overview of Results (28 Tage) - μg/m3
<15mg/kg
TVOC (C6 - C16) - μg/m3
8. References
EN 1602
EN 1602: 2013: Thermal insulating products for ISO 14040
building applications - Determination of the apparent ISO 14040: Environmental management — Life cycle
density assessment — Principles and framework
EN ISO 8497 ISO 14044
EN ISO 8497: Thermal insulation - Determination of ISO 14044: Environmental management — Life cycle
steady-state thermal transmission properties of thermal assessment — Requirements and guidelines
insulation for circular pipes
EN 14707
ISO 9001 EN 14707: 2012: Thermal insulating products for
ISO 9001: 2015: Quality management systems. building equipment and industrial installations.
Determination of maximum service temperature for
EN 13501-1 preformed pipe insulation
EN 13501-1:2007+A1: 2013 Fire classification of
construction products and building elements - EN 15804
Classification using test data from reaction to fire tests EN 15804: 2012-04 + A1 2014: Sustainability of
construction works — Environmental Product
ISO 14001 Declarations — Core rules for the product category of
ISO 14001: 2015 Environmental management construction products
systems.
CEN/TR 15941
EN ISO 14025 CEN/TR 15941: Sustainability of construction works -
EN ISO 14025: 2011-10: Environmental labels and Environmental product declarations - Methodology for
declarations — Type III environmental declarations — selection and use of generic data
Principles and procedures
9 Environmental Product Declaration NMC sa – CLIMAFLEX®naturefoam easy
CEN TS 16516 Instructions for the EPD Programme of Institut Bauen
CEN TS 16516: /AgBB/, /ISO 16000-3/, /ISO 16000-6/, und Umwelt e.V., Version 2.0 2021
/ISO16000-9/, /ISO 16000-11/ Construction products -
Assessment of release of dangerous substances. Product Category Rules for Building-Related
Determination of emissions into indoor air Products and Services
Institute Construction and Environment e.V. (IBU)
EN 16783 Part A: Calculation Rules for the Life Cycle
EN 16783: 2017 Thermal insulation products - Product Assessment and Requirements on the Project Report
category rules (PCR) for factory made and in-situ Version 1.7
formed products for preparing environmental product
declarations PCR Guidance-Texts for Building-Related Products
and Services
Eurostat From the range of Environmental Product Declarations
European Statistics: Recovery rates for packaging of Institute Construction and Environment e.V. (IBU)
waste Paper and cardboard packaging for the Part B: Requirements on the EPD for Insulating
European Union 27 countries 2014 materials made of foam plastics
http://ec.europa.eu/eurostat/home Version 1.6 (Template) Version 1.2 (PCR specific)
Eurofins Sphera
Eurofins: Product Testing Institute Sphera Solutions Gmbh. GaBi 10 LCI documentation.
GaBi Databases (sphera.com) Stuttgart,
Gabi ts Echterdingen: Sphera Solutions Gmbh
GaBi 10 GaBi Software-System and Database for Life
Cycle Engineering Copyright © 1992-2021 Sphera
Solutions Gmbh Version: 10.5.0.78 DB Schema 8007
Institut Bauen und Umwelt
Institut Bauen und Umwelt e.V., Berlin(pub.): General
10 Environmental Product Declaration NMC sa – CLIMAFLEX®naturefoam easy
Publisher
Institut Bauen und Umwelt e.V. Tel +49 (0)30 3087748- 0
Panoramastr. 1 Fax +49 (0)30 3087748- 29
10178 Berlin Mail info@ibu-epd.com
Germany Web www.ibu-epd.com
Programme holder
Institut Bauen und Umwelt e.V. Tel +49 (0)30 - 3087748- 0
Panoramastr 1 Fax +49 (0)30 – 3087748 - 29
10178 Berlin Mail info@ibu-epd.com
Germany Web www.ibu-epd.com
Author of the Life Cycle
Assessment Tel +32 (0) 87 85 85 00
NMC S.A. Fax +32 (0) 87 85 85 11
Gerd-Noël-Strasse 1 Mail info@nmc.eu
4731 Eynatten Web www.nmc.eu
Belgium
Owner of the Declaration
NMC S.A. Tel +32 (0) 87 85 85 00
Gerd-Noël-Strasse 1 Fax +32 (0) 87 85 85 11
4731 Eynatten Mail info@nmc.eu
Belgium Web www.nmc.eu
