ENVIRONMENTAL PRODUCT DECLARATION
as per ISO 14025 and EN 15804+A2
Owner of the Declaration Hansgrohe Group
Publisher Institut Bauen und Umwelt e.V. (IBU)
Programme holder Institut Bauen und Umwelt e.V. (IBU)
Declaration number EPD-HAN-20240195-ICC1-EN
Issue date 03.12.2024
Valid to 02.12.2029
Shower Sets Standard
Hansgrohe Group
www.ibu-epd.com | https://epd-online.com
1. General Information
Hansgrohe Group Shower Sets Standard
Programme holder Owner of the declaration
IBU – Institut Bauen und Umwelt e.V. Hansgrohe Group
Hegelplatz 1 Auestr. 5-9
10117 Berlin 77761 Schiltach
Germany Germany
Declaration number Declared product / declared unit
EPD-HAN-20240195-ICC1-EN One piece of an average shower set (standard).
This declaration is based on the product category rules: Scope:
Fittings and showers, 01.08.2021 This average EPD covers the most relevant chrome plated shower sets
(PCR checked and approved by the SVR) based on criteria like sales volume, long-term relevance and price point.
The owner of the declaration shall be liable for the underlying information
and evidence; the IBU shall not be liable with respect to manufacturer
Issue date information, life cycle assessment data and evidences.
03.12.2024
The EPD was created according to the specifications of EN 15804+A2. In
the following, the standard will be simplified as EN 15804.
Valid to
Verification
02.12.2029
The standard EN 15804 serves as the core PCR
Independent verification of the declaration and data according to ISO
14025:2011
internally X externally
Dipl.-Ing. Hans Peters
(Chairman of Institut Bauen und Umwelt e.V.)
Florian Pronold Dr Naeem Adibi,
(Managing Director Institut Bauen und Umwelt e.V.) (Independent verifier)
1 Environmental Product Declaration - Hansgrohe Group - Shower Sets Standard
2. Product
Name Value Unit
2.1 Product description/Product definition
Brass 26.5 %
Shower sets essentially comprise of hand shower, shower hose
Plastic 23.0 %
plus shower bar.
Cardboard, Paper 20.9 %
A hand shower consists of a housing made of plastic materials PVC 15.4 %
or metal and a jet disc as well as several assembly parts of ABS 10.0 %
various materials. A shower hose is a plastic hose with metal
Coating metals 1.8 %
connectors, made of brass or stainless steel. The shower bar
Stainless Steel 1.3 %
surface is usually chrome-plated by means of various galvanic
process stages. Zinc 0.9 %
Other material 0.1 %
For the use and application of the product the respective
national provisions at the place of use apply, in Germany for
The parts which are made of brass contain between 0.2 and
example the building codes of the federal states and the
1.4% lead.
corresponding national specifications.
This product contains substances listed in the candidate list
The products comply with the applicable standards and
(date: 17.12.2021) exceeding 0.1 percentage by mass: Lead
regulations listed below.
(CAS number 7439-92-1) as a component of the brass alloy
has been on the candidate list of the Reach Regulation
Following standards apply to all shower sets to prove product
(Regulation (EC) No. 1907/2006) since 27.06.2018.
safety:
• EN 1112:2008: Sanitary tapware – Shower outlets for This product/article/at least one partial article contains other
sanitary tapware for water supply systems of type 1 and CMR substances in categories 1A or 1B which are not on the
type 2 candidate list, exceeding 0.1 percentage by mass: no.
• EN 1113:2015: Sanitary tapware – Shower hoses for
sanitary tapware for water supply systems of type 1 and Biocide products were added to this construction product or it
type 2 has been treated with biocide products (this then concerns a
• ISO 3822: Acoustics – Laboratory tests on noise treated product as defined by the (EU) Ordinance on Biocide
emission from appliances and equipment used in water Products No. 528/2012): no.
supply installations
2.6 Manufacture
2.2 Application Hand shower:
Shower sets are a combination of a hand shower, a shower
hose and a shower bar. The shower bar enables the shower
head to be fixed at any height. They are used in bathrooms for
showering or in bathtubs.
2.3 Technical Data
Constructional data
Name Value Unit
Maximum load temperature
42 °C
permanent operation
Maximum load temperature
70 °C
temporary operation
Flow rate (indications for Depending on flow rate
m3/h
pressure range of 1-3 bar) class 0,571 to 1,02
Sound emissions <30 dB
Performance data of the product with respect to its
characteristics in accordance with the relevant technical
provision (no CE-marking).
2.4 Delivery status
The shower sets are delivered singularly packaged. The No. 1: The plastic handle of the hand showers is injected.
packaging is customized to the size of the product and No. 2: The handle is galvanized with chrome.
supplies. Customers can order single products or multiple No. 3: The plastic inlet housing is injected.
products with outer packaging. The products with the smallest No. 4: The plastic pipe bow is injected.
and the largest volume have dimensions between 730x152x65 No. 5: The plastic distributor is injected.
mm and 990x165x75 mm. No. 6: Meanwhile, the plastic jet body is injected.
No. 7: The distributor and the jet body are preassembled.
2.5 Base materials/Ancillary materials No. 8: All the parts are assembled and packed.
The material composition (incl. packaging) of an average
shower set is as follows: Shower hose:
2 Environmental Product Declaration - Hansgrohe Group - Shower Sets Standard
recycled material. The cardboard is always printed with lead-
free ink and clear dispersion varnish. The inlay of the packaging
consists of folded cardboard, fiber form or plastic bags,
depending on the product. The packaging can be fully recycled.
2.10 Condition of use
To protect the shower sets and make them durable, the product
is usually chrome-plated. Nevertheless, it will not release
unhealthy contaminants in the water, if used as intended. To
ensure the longevity of the product, it should be used and
cleaned regularly.
2.11 Environment and health during use
Our products do not emission any contaminants or substances
that are harmful to the environment or health during the use
phase.
2.12 Reference service life
The quality and durability of our shower sets is designed for a
product life of about 20 years. Which on average is
approximately the duration of use by the consumers.
No. 1: The TPE inner tube is extruded.
Nevertheless, it is possible that some parts are needed to be
No. 2: The PVC top layer is applied on the inner tube.
changed earlier (like shower hoses).
No. 3: The embossing foil chrome is applied on the top layer.
No. 4: The hose is cut in length and assembled with the
With few exceptions, all products have a five-year warranty.
connections.
Furthermore, an after-sale service warranty of 15 years is
provided.
Packaging:
In the end all components are packed together with some
additional parts like shower bar and slider. 2.13 Extraordinary effects
Fire
Any production waste generated is disposed accordingly. In
The products are not classified as building materials (building
individual cases, the production may differ slightly from the
products) and are not subject to DIN 4102 and EN 13501-1.
procedure
Fire protection
2.7 Environment and health during manufacturing Name Value
Hansgrohe SE tries to keep the impact on people and the Building material class -
environment as low as possible when manufacturing its
Burning droplets -
products.
Smoke gas development -
Hazards at workplaces are regularly assessed and reduced to a
minimum.
For example, in basic production, sawing or grinding work is Water
mainly carried out by robots, and in electroplating, chemicals If a room in which the products offered by Hansgrohe are
are dosed automatically via appropriate pump stations. installed is flooded with water, the products are not affected in
Emissions that are hazardous to health are extracted directly at their function. There will be no environmental impact.
the source and cleaned by filter systems.
Workplace and emission limits are regularly monitored and are Mechanical destruction
far below the prescribed limits. If the surface of the coating is destroyed by a mechanical
To reduce environmental impact, water and production waste stress, there is a possibility of corrosion. In the event of
are recycled wherever possible. mechanical damage, the products may need to be replaced
In addition, all production sites are certified according to the due to possible sharp cut edges.
DIN EN ISO standards 14001 (environment), 50001 (energy),
45001 (occupational health and safety) and 9001 (quality). 2.14 Re-use phase
Continuous improvement of environmental and occupational The shower sets are not taken back by the manufacturer for the
safety performance is thus guaranteed. purpose of reuse. Users can disassemble the products
repeatedly within the reference utilization period and reuse it
2.8 Product processing/Installation elsewhere.
Make holes in the wall for the fixation of the shower bar (tool:
drilling machine) and insert dowels and silicone (tool: silicon 2.15 Disposal
injector). The waste code of the product is AVV 20 03 01. Disassembly of
Screw on the shower bar (tool: screwdriver) and attach the the products consists of the same steps as assembly, in
cover caps. reverse order. All metal components can be recycled (as
Screw the shower hose with union nut and seal onto the wall scrap).All plastic components have a high calorific value and
outlet by hand. can be sent for thermal recycling. In countries where no thermal
Screw the shower hose with union nut and seal onto the hand recycling or substance recycling is established, disposal takes
shower by hand. place via the waste incineration plant.
2.9 Packaging 2.16 Further information
For product protection the shower sets are individually packed Additional information about our products can be found at
in a cardboard box, which consists of approximately 80% https://www.hansgrohe.com.
3 Environmental Product Declaration - Hansgrohe Group - Shower Sets Standard
3. LCA: Calculation rules
C3) in the form of the average European electricity mix or
3.1 Declared Unit thermal energy from natural gas. Recycling of paper, plastic
The results of this EPD are valid for the following functional and metal scrap results in credits of the respective raw
unit: materials for the primary material portion of the input. The loads
Provide sanitary function for one (1) average shower set unit of the waste incineration and recycling processes are assigned
used in accordance with the manufacturer's recommendations to the respective modules (A3, A5 and C3) and not to module
for a 20-year life, following the manufacturer's operating D.
instructions. An average conditioned shower set is considered
the baseline flow. 3.3 Estimates and assumptions
Energy and water consumption, material amount for coating as
Weighted averaging based on production tonnages in 2022/23 well as waste during production could only be determined on
is chosen as basis for creating the environmental profile. 26 concrete, existing products and not on the average product.
different shower sets were considered. The highest value of all inputs and outputs for energy, waste
and coating of the top seller, the lightest and the heaviest
Declared unit
product was used for the calculation of energy, water, waste
Name Value Unit
and coating.
Declared unit 1 pce. For the incineration with energy recovery (thermal and electric)
Declared unit with packaging 1.206 kg of waste, an r1 value of > 0.6 is assumed. The net efficiency for
Packaging 0.271 kg the average waste incinerated is between 38 % and 44 %,
depending on the type of waste respectively the disposal data
Weight range of the products 1.078-1.62 kg
set.
Mass reference 1.206 kg/pce
3.4 Cut-off criteria
The effect associated with the neglected mass shares is less
3.2 System boundary than 5% of the effect categories per module. The minimum limit
This representative EPD follows the EPD type "cradle to gate - of 1% total mass and the use of renewable and nonrenewable
with options". The following life cycle modules are declared: primary energy is not exceeded.
Modules A1-A3:
3.5 Background data
The product stage begins with considering the production of the
necessary raw materials and energies, including all The LCA software LCA for Experts (GaBi) 10.7 was used to
corresponding upstream chains and the actual procurement model the life cycle. The entire manufacturing process, as well
transports. Furthermore, the entire manufacturing phase was as energy consumption, were modelled on the basis of
mapped, including the treatment of production waste until the manufacturer specific data. However, generic background
end-of- waste status (EoW) was reached. Green electricity from datasets were used for the upstream and downstream
hydropower is used for the manufacturing processes in processes. The majority of the background datasets used were
Germany. Green electricity from hydropower and wind power taken from the current version (2023.2) of the GaBi database.
(50% each) is used for the French production site. US electricity Ecoinvent Version 3.9 (2021) datasets were only used when
mix is used for the US production site. suitable GaBi datasets were not available.
Module A4:
3.6 Data quality
All distribution transports to the customers were considered.
The background datasets used for accounting purposes mainly
Module A5:
originate from the respective updated GaBi databases at the
This module covers the installation process with the
time of calculation. The data for the examined products was
corresponding packaging waste generated that needs to be
captured on the basis of evaluations of internal production and
disposed.
environmental data, the collection of LCA relevant data within
Modules B1 & B3-B5:
the supply chain, as well as the evaluation of relevant data for
These modules were considered, but evaluated as not relevant
the energy supply. The collected data were checked for
for the products and considered as zero.
plausibility and consistency.
Module B2:
Good representativity can be assumed.
Maintenance expenses are declared in this module and consist
For the assessment of the variability of the results, all products
of weekly cleaning expenses for this product.
were balanced in addition to the average product. See at
Module B6:
chapter 6 for explanation of the variability.
This module considers the energy input required to bring water
to a certain temperature for the use of a gas low temperature
3.7 Period under review
boiler (scenario B6/1) and for the use of an electric
Life cycle assessment data were collected in 2022/23.
instantaneous water heater (scenario B6/2).
Module B7: 3.8 Geographic Representativeness
This module considers the water consumption that can be
Land or region, in which the declared product system is
expected depending on the function of the product family.
manufactured, used or handled at the end of the product´s
Modules C1-C4:
lifespan: Europe
The modules include the environmental impacts for dismantling
of the products and the treatment of the waste fractions until
the end-of-waste status (EoW) is reached, including the 3.9 Allocation
associated transports at the end of the product life cycle. For the production process nearly all raw materials, precursors
Module D: and supplies could be assigned to the declared product.
Identification of the benefits and costs of the product outside Energy, water, galvanization process and production waste
the system boundary. For waste, paper and plastics, these were assigned to the highest value of either the heaviest,
consist of energy credits from thermal utilization (A3, A5 and lightest or most sold product of the product group. No
4 Environmental Product Declaration - Hansgrohe Group - Shower Sets Standard
byproducts are produced and no allocation is required. considered, based on Eurostat.
Some of the brass losses from brass processing in module A3 Deconstructed product at the end of life:
are directly reused by Hansgrohe and are modelled as a closed Since the product has a high plastic content, it is assumed that
loop. Another part of the brass losses (brass particles and 95% of the plastic and metal components are incinerated (C3)
dusts) is disposed of as waste (without debits and credits). and 5% are disposed in landfill (C4). The metal components are
Credits for plastics, paper and cardboard recycled in A5 and incinerated without energy recovery and the plastic
metallurgical waste in C3 are credited in module D. components are incinerated with energy recovery.
Credits for the energy recovery of incinerated production waste
in A1-3, paper, cardboard and plastics in A5 and plastics and 3.10 Comparability
other materials in C3 are credited in module D. Basically, a comparison or an evaluation of EPD data is only
The loads for waste water treatment and waste disposal of core possible if all the data sets to be compared were created
sand, waste oil and hazardous waste from the manufacturing according to EN 15804 and the building context, respectively
phase are allocated to module A3. the product-specific characteristics of performance, are taken
Packaging: into account. The background database used is LCA for
For paper and cardboard, recycling (91 %) and energy recovery Experts (GaBi) 10.7 in the
(9 %) are considered on a pro rata basis. For plastic, a database version 2023.2.
proportionate recycling (52 %), energy recovery (48 %)
4. LCA: Scenarios and additional technical information
Characteristic product properties of biogenic carbon
Service life
The biogenic carbon content was calculated based on the
Hansgrohe SE declares a Service Life of 20 years as an
factors from the Thünen Intitute.
empirical value for the shower sets ECOsmart when used in
Information on describing the biogenic carbon content at accordance with the care instructions. This value is based on
factory gate their technical service centre's statistics on service life in the
Name ValueUnit market and complaints.
kg Name Value Unit
Biogenic carbon content in product -
C Life Span according to the manufacturer 20 a
Biogenic carbon content in accompanying kg
0.103
packaging C Operational energy use (B6) and Operational water use
(B7)
Note: 1 kg of biogenic carbon is equivalent to 44/12 kg of CO2.
Modules B6 and B7 are calculated based on the directions of
the IBU PCR part B.
Module B6 considers the operational energy use. Scenario B6
The following technical information is a basis for the declared
assumes the use of a gas low temperature boiler. Scenario
modules.
B6/1 assumes the use of an electric instantaneous water heater
Transport to the building site (A4) (21 kW). Module B7 considers the operational water use.
Name Value Unit Name Value Unit
Transport distance (Truck) 607 km Water consumption 102.7 m3
Capacity utilisation (including empty runs) 55 %
Energy demand 4779 kWh
Transport distance (Container ship) 1460 km
Capacity utilisation (Container ship) 80 % End of life (C1-C4)
Name Value Unit
Installation into the building (A5)
Collected separately waste type 0.956 kg
No additional resources or energy are required for the
Energy recovery 0.909 kg
installation. The packaging is disposed either by recycling or
Landfilling 0.047 kg
incineration.
Name Value Unit
Reuse, recovery and/or recycling potentials (D), relevant
Packaging (Paper, cardboard, plastic) 0.271 kg
scenario information
Maintenance (B2) The energy generated from energy recovery as well as recycled
For module B2, it is assumed that a weekly cleaning of the materials are assigned to module D as possible potentials or
product takes place, with 0.5 liter of water containing 1.5% avoided loads in subsequent systems. Credits are only given
soap. for the primary portion of the inputs.
Name Value Unit
Maintenance cycle (cleaning) 780 Number/RSL
Water consumption/Cyle weekly (cleaning) 0.5 Liter/cycle
Soap concentration (cleaning) 1.5 %
Water consumption (cleaning) 0.52 m3
Auxiliary Soap/Tensides (cleaning) 7.8 kg
5 Environmental Product Declaration - Hansgrohe Group - Shower Sets Standard
5. LCA: Results
The following table shows the result of the LCA for 1 piece of an average shower set. The results in the B-module are based on a
lifetime of 20 years. Scenario B6 shows the result for the use of a gas low temperature boiler. Scenario B6/1 shows the result for the
use of an electric instantaneous water heater.
DESCRIPTION OF THE SYSTEM BOUNDARY (X = INCLUDED IN LCA; MND = MODULE OR INDICATOR NOT DECLARED; MNR
= MODULE NOT RELEVANT)
Benefits and
Construction loads beyond
Product stage Use stage End of life stage
process stage the system
boundaries
la ire ta m w a Ry lp p u s tro p s n a rT g n iru tc a fu n a M e h t m o rf tro p s n a rTe tis e h t o t e ta g y lb m e s s A e s U e c n a n e tn ia M ria p e R tn e m e c a lp e R tn e m h s ib ru fe R y g re n e la n o ita re p Oe s u re ta w la n o ita re p Oe s u n o itc u rts n o c -e Dn o itilo m e d tro p s n a rT g n is s e c o rp e ts a W la s o p s iD -e s u e R-y re v o c e R-g n ilc y c e Rla itn e to p
A1 A2 A3 A4 A5 B1 B2 B3 B4 B5 B6 B7 C1 C2 C3 C4 D
X X X X X X X X X X X X X X X X X
RESULTS OF THE LCA - ENVIRONMENTAL IMPACT according to EN 15804+A2: 1 piece average shower set (standard)
Parameter Unit A1-A3 A4 A5 B1 B2 B3 B4 B5 B6 B6/1 B7 C1 C2 C3 C4 D
GWP-total kg CO 2 3.46E 9.72E- 5.54E- 0 2.42E 0 0 0 1.27E 1.54E 5.52E 0 1.82E- 1.34E 2.84E-03 -9.69E-
eq +00 02 01 +01 +03 +03 +01 02 +00 01
GWP-fossil kg CO 2 3.83E 9.65E- 1.76E- 0 1.82E 0 0 0 1.27E 1.54E 5.52E 0 1.8E-02 1.34E 2.83E-03 -5.96E-
eq +00 02 01 +01 +03 +03 +01 +00 01
GWP- kg CO 2 -3.78E- 0 3.78E- 0 0 0 0 0 0 0 0 0 0 0 0 -3.74E-
biogenic eq 01 01 01
GWP-luluc kg CO 2 4.9E-03 7.17E- 1.85E- 0 6.02E 0 0 0 4.34E- 1.68E- 1.57E- 0 1.66E- 1.12E- 2.53E-06 4.02E-05
eq 04 04 +00 02 01 02 04 04
kg CFC11 1.14E- 8.12E- 1.09E- 2.81E- 2.84E- 3.64E- 2.34E- 1.04E- -7.28E-
ODP 5.86E-10 0 0 0 0 0 4.75E-15
eq 14 13 06 10 08 10 15 10 10
7.61E- 4.75E- 6.64E- 3.29E 1.37E- 2.92E- 5.73E-
AP mol H+ eq 3.08E-02 0 0 0 0 7.7E-01 0 8.74E-06 2.28E-05
04 04 02 +00 01 05 04
EP- 2.87E- 3.17E- 5.81E- 1.28E- 5.75E- 6.48E- 6.57E- 2.21E-
kg P eq 2.18E-05 0 0 0 0 0 3.79E-07 -3.4E-06
freshwater 07 07 04 04 03 02 08 07
2.04E- 1.08E- 1.51E- 3.34E- 7.88E- 1.13E- 2.46E- -2.05E-
EP-marine kg N eq 2.41E-03 0 0 0 0 2.8E-01 0 2.08E-06
04 04 02 01 01 05 04 04
2.26E- 1.18E- 1.81E- 3.65E 8.23E 4.09E- -2.16E-
EP-terrestrial mol N eq 2.5E-02 0 0 0 0 0 1.3E-04 2.9E-03 2.27E-05
03 03 01 +00 +00 01 03
kg
5.54E- 3.67E- 6.03E- 1.04E- 6.47E- -4.96E-
POCP NMVOC 8.58E-03 0 0 0 0 9.7E-01 2.1E+00 0 2.6E-05 6.56E-06
04 04 02 01 04 04
eq
2.69E- 1.54E- 2.38E- 2.59E- 1.19E- 7.92E-
ADPE kg Sb eq 3.05E-04 5.3E-09 0 2.1E-05 0 0 0 0 7.6E-11 3.59E-05
06 05 04 06 09 09
7.43E 1.28E 2.49E 4.52E 2.14E 3.24E 6.16E 2.45E- 1.33E
ADPF MJ 0 0 0 0 0 4.23E-02 -1E+01
+01 +00 +00 +02 +04 +04 +02 01 +00
m3 world
9.66E- 5.41E- 6.94E 4.14E 3.44E 1.92E 2.17E- -3.77E- -3.19E-
WDP eq 4.36E-02 0 0 0 0 0 1.3E-01
04 02 +00 +00 +02 +01 04 05 03
deprived
GWP = Global warming potential; ODP = Depletion potential of the stratospheric ozone layer; AP = Acidification potential of land and water; EP =
Eutrophication potential; POCP = Formation potential of tropospheric ozone photochemical oxidants; ADPE = Abiotic depletion potential for non-fossil
resources; ADPF = Abiotic depletion potential for fossil resources; WDP = Water (user) deprivation potential)
RESULTS OF THE LCA - INDICATORS TO DESCRIBE RESOURCE USE according to EN 15804+A2: 1 piece average shower set
(standard)
Parameter Unit A1-A3 A4 A5 B1 B2 B3 B4 B5 B6 B6/1 B7 C1 C2 C3 C4 D
1.73E 9.38E 2.11E 1.94E 2.32E -4.44E
PERE MJ 7.77E-02 5.4E+00 0 0 0 0 0 1.78E-024.16E-01 3.83E-03
+01 +01 +02 +04 +02 +00
4.17E -4.17E
PERM MJ 0 0 0 0 0 0 0 0 0 0 0 0 0 0
+00 +00
2.14E 9.38E 2.11E 1.94E 2.32E -4.44E
PERT MJ 7.77E-021.23E+00 0 0 0 0 0 1.78E-024.16E-01 3.83E-03
+01 +01 +02 +04 +02 +00
5.63E 1.29E 4.52E 2.14E 3.25E 6.16E 1.79E
PENRE MJ 3.1E+00 0 0 0 0 0 2.46E-01 9.15E-01 -1E+01
+01 +00 +02 +04 +04 +02 +01
1.81E -6.08E- -1.66E -8.73E-
PENRM MJ 0 0 0 0 0 0 0 0 0 0 0 0
+01 01 +01 01
7.44E 1.29E 4.52E 2.14E 3.25E 6.16E 1.33E
PENRT MJ 2.49E+00 0 0 0 0 0 2.46E-01 4.23E-02 -1E+01
+01 +00 +02 +04 +04 +02 +00
SM kg 5.23E-01 0 0 0 0 0 0 0 0 0 0 0 0 0 0 3.91E-02
RSF MJ 1.52E-23 0 0 0 0 0 0 0 0 0 0 0 0 0 0 0
NRSF MJ 1.78E-22 0 0 0 0 0 0 0 0 0 0 0 0 0 0 0
6 Environmental Product Declaration - Hansgrohe Group - Shower Sets Standard
1.57E -1.53E-
FW m3 1.97E-028.53E-05 1.8E-03 0 1.62E-01 0 0 0 2.04E-01 5.41E-01 0 1.95E-053.21E-03 4.82E-07
+01 03
PERE = Use of renewable primary energy excluding renewable primary energy resources used as raw materials; PERM = Use of renewable primary
energy resources used as raw materials; PERT = Total use of renewable primary energy resources; PENRE = Use of non-renewable primary energy
excluding non-renewable primary energy resources used as raw materials; PENRM = Use of non-renewable primary energy resources used as raw
materials; PENRT = Total use of non-renewable primary energy resources; SM = Use of secondary material; RSF = Use of renewable secondary fuels;
NRSF = Use of non-renewable secondary fuels; FW = Use of net fresh water
RESULTS OF THE LCA – WASTE CATEGORIES AND OUTPUT FLOWS according to EN 15804+A2:
1 piece average shower set (standard)
Parameter Unit A1-A3 A4 A5 B1 B2 B3 B4 B5 B6 B6/1 B7 C1 C2 C3 C4 D
-2.54E- -1.42E-
HWD kg 3.12E-06 4E-12 8.04E-11 0 8.5E-03 0 0 0 3.72E-06 0 7.61E-131.32E-103.53E-121.84E-07
06 08
3.34E 2.38E
NHWD kg 3.93E-011.82E-043.42E-02 0 6.59E-01 0 0 0 1E+02 0 3.75E-05 5.1E-02 4.77E-021.98E-02
+00 +01
5.16E -4.75E-
RWD kg 1.31E-032.25E-061.27E-04 0 4.14E-03 0 0 0 4.94E-02 5.3E-02 0 4.6E-07 5.46E-054.98E-07
+00 04
CRU kg 0 0 0 0 0 0 0 0 0 0 0 0 0 0 0 0
MFR kg 0 0 2.38E-01 0 0 0 0 0 0 0 0 0 0 0 0 0
MER kg 0 0 0 0 0 0 0 0 0 0 0 0 0 0 0 0
2.39E
EEE MJ 1.88E-01 0 1.08E-01 0 0 0 0 0 0 0 0 0 0 2.31E-05 0
+00
4.31E
EET MJ 3.7E-01 0 1.94E-01 0 0 0 0 0 0 0 0 0 0 0 0
+00
HWD = Hazardous waste disposed; NHWD = Non-hazardous waste disposed; RWD = Radioactive waste disposed; CRU = Components for re-use;
MFR = Materials for recycling; MER = Materials for energy recovery; EEE = Exported electrical energy; EET = Exported thermal energy
RESULTS OF THE LCA – additional impact categories according to EN 15804+A2-optional:
1 piece average shower set (standard)
Parameter Unit A1-A3 A4 A5 B1 B2 B3 B4 B5 B6 B6/1 B7 C1 C2 C3 C4 D
Disease
PM ND ND ND ND ND ND ND ND 4.93E-06 2.77E-05 ND ND ND ND ND ND
incidence
kBq U235
IR ND ND ND ND ND ND ND ND 8.02E+008.58E+02 ND ND ND ND ND ND
eq
ETP-fw CTUe ND ND ND ND ND ND ND ND 2.64E+029.02E+03 ND ND ND ND ND ND
HTP-c CTUh ND ND ND ND ND ND ND ND 6.91E-08 4.77E-07 ND ND ND ND ND ND
HTP-nc CTUh ND ND ND ND ND ND ND ND 6.71E-06 7.61E-06 ND ND ND ND ND ND
SQP SQP ND ND ND ND ND ND ND ND 1.51E+021.27E+04 ND ND ND ND ND ND
PM = Potential incidence of disease due to PM emissions; IR = Potential Human exposure efficiency relative to U235; ETP-fw = Potential comparative
Toxic Unit for ecosystems; HTP-c = Potential comparative Toxic Unit for humans (cancerogenic); HTP-nc = Potential comparative Toxic Unit for humans
(not cancerogenic); SQP = Potential soil quality index
Disclaimer 1 – for the indicator 'Potential Human exposure
efficiency relative to U235'. This impact category deals mainly with the eventual impact of low-dose ionizing radiation on human health
of the nuclear fuel cycle. It does not consider effects due to possible nuclear accidents, occupational exposure or radioactive waste
disposal in underground facilities. Potential ionizing radiation from the soil, radon and from some construction materials is also not
measured by this indicator.
Disclaimer 2 – for the indicators 'abiotic
depletion potential for non-fossil resources', 'abiotic depletion potential for fossil resources', 'water (user) deprivation potential,
deprivation-weighted water consumption', 'potential comparative toxic unit for ecosystems', 'potential comparative toxic unit for humans
– cancerogenic', 'Potential comparative toxic unit for humans - not cancerogenic', 'potential soil quality index'. The results of this
environmental impact indicator shall be used with care as the uncertainties on these results are high as there is limited experience with
the indicator.
6. LCA: Interpretation
7 Environmental Product Declaration - Hansgrohe Group - Shower Sets Standard
of the variability of the results, all products were balanced and
compared to the average product weighted by production
volume.
The dominance analysis shows that modules B2, B6 and B7 The different types of products all have the same function and
are the dominant life cycle stages in most of the categories. differ mainly in terms of design, which has an influence on
The contribution of B2 is due to the demand of soap and water construction and materials used. The basic structure of the
for cleaning. Module B6 dominates most of the indicators due product types is always similar. Material type and quantity
to the energy demand for water heating and module B7 has a proportions do not differ much, as also shown in the average
high contribution to EPfreshwater due to the wastewater material composition table.
treatment. The module A1-A3 has a very low contribution to all The deviation of the GWP fossil in modules A1-C4 has a
categories except of ADPE. In this indicator the provision of maximum of 17% and a minimum of -5% with a mix scenario of
brass has the largest contribution. The end-of-life stage has no 50% B6/1 and 50% B6/2. The deviation of the PENRT in
significant influence on the environmental indicators. modules A1-C4 has a maximum of 17% and a minimum of -5%.
The environmental burdens from the transports (modules A4 The deviation of the NHWD in modules A1-C4 has a maximum
and C2) account for less than 0.1% of the total burdens of the of 17% and a minimum of -5%. Modules B6 and B7 account for
respective indicators in all cases. more than 90% of the GWP indicator. The deviation from the
The possible potentials of avoided loads of subsequent average is mainly caused by the flow rate in module B7. The
systems (module D) lie outside the considered system higher the deviation from the average GWP, the higher the flow
boundaries and relate exclusively to credits from recycling and rate. The flow rate ranges between 13.8 and 17 l/min.
thermal recycling by means of incineration with energy recovery Consequently, the production phase has a minor influence on
of the different materials. the LCA results.
12 different product types were produced. For the assessment
7. Requisite evidence
The drinking water regulation determines the quality of drinking • Elastomer guideline: Guideline for the hygienic
water at the point of withdrawal. This results in requirements for assessment of elastomers in contact with drinking water
used materials in drinking water installations in general and • Thermoplastic elastomers: Recommendation for the
therefore in sanitary fittings in particular. hygienic assessment of products made of thermoplastic
All materials used by Hansgrohe SE, which are in contact with elastomers in contact with drinking water (TPE transition
drinking water, fulfill the drinking water regulation. recommendation)
• Ceramics: draft assessment basis for enamels and
Regulations for metals (Europe-wide): ceramic materials: assessment basis for enamels and
ceramic materials in contact with drinking water
• Acceptance of metallic materials used for products in
(enamel/ceramic assessment basis)
contact with drinking water: 4MS Common Approach
• Lubricants: Guideline for the hygienic assessment of
- Part A – Procedure for the acceptance
lubricants in contact with drinking water (sanitary
- Part B – 4MS Common Composition List
lubricants), (Lubricant Guideline)
• Metal recommendation of the federal environment
agency: metal materials suitable for drinking water
Regulation for other materials (France):
hygiene
• ACS: Attestation de Conformité Sanitaire (plastics,
Regulations for other materials (Germany): elastomers)
• KTW: Assessment basis for plastics and other organic
Regulation for other materials (UK):
materials in contact with drinking water
8 Environmental Product Declaration - Hansgrohe Group - Shower Sets Standard
elastomers)
• BS 69 20: Suitability of non-metallic products for use in
contact with water intended for human consumption with
Products of the Hansgrohe SE are therefore uncritical to use
regard to their effect on the quality of water (plastics,
with any drinking water.
8. References
Standards AVV
Draft General administrative provision relating to the Order on
EN 1112 the European list of wastes (Waste List Order – German
EN 1112:2008 Sanitary tapware - Shower designation: AVV) of 10 December 2001.
outlets for sanitary tapware for water supply systems of type 1
and type 2 - General technical specification ECHA
European Chemicals Agency (ECHA) Candidate List of
ISO 3822 Substances of Very High Concern (SVHC) for Authorisation
ISO 3822: Acoustics – Laboratory tests on noise emission from https://echa.europa.eu/de/candidate-listtable
appliances and equipment used in water supply installations
Ecoinvent
DIN 4102-1 ecoinvent 3.9 Database on Life Cycle Inventories (Life Cycle
DIN 4102-1: Fire behaviour of building materials and building Inventory data), ecoinvent Association, Zürich, 2021
components - Part 1: Building materials; concepts,
requirements and tests. 1998-05 EU Ordinance on biocide Products No. 528/2012
European Parliament, 2012. Regulation (EU) no528/2012 of the
DIN EN ISO 9001 European parliament and of thecouncil of 22 May 2012
DIN EN ISO 9001:2015: Quality management systems - concerning the makingavailable on the market and use of
Requirements (ISO 9001:2015) biocidal products
DIN EN 13501-1 Eurostat
DIN EN 13501-1:2019-05: Fire classification of construction Eurostat, last update 26/10/2021 on
products and building elements - Part 1:Classification using https://ec.europa.eu/eurostat/databrowser/view/ten00063/default/table?
data from reaction to fire tests; German version EN 13501- ang=en
1:2018
LCA for Experts
DIN EN ISO 14001 LCA for Experts (GaBi) 10.7, GaBi Software System and
DIN EN ISO 14001:2015, Environmental management systems Database for Life Cycle Engineering version 2023.2, Sphera
— Requirements with guidance for use, 2015- 09 Solutions GmbH, Leinfelden-Echterdingen, 1992-2023
DIN EN ISO 14025 IBU 2021
DIN EN ISO 14025: Environmental labels and declarations - General Instructions for the EPD programme of Institut Bauen
Type III environmental declarations - Principles and procedures, und Umwelt e.V. Version 2.0, Berlin: Institut Bauen und Umwelt
2011-10 e.V., 2021, www.ibu-epd.com
EN 15804 PCR Part A
DIN EN 15804:2012+A2:2019+AC:2021: Sustainability of Institut Bauen und Umwelt e.V. (IBU), Product Category Rules
construction works - Environmental product declarations - Core for Building-Related Products and Services. Part A: Calculation
rules for the product category of construction products rules for the life cycle 11 Environmental Product Declaration
Hansgrohe Group – Hand Showers assessment and
DIN EN ISO 45001 requirements on the project report. Version 2.1, Berlin, 11/2021
DIN EN ISO 45001:2018: Occupational health and safety
management systems — Requirements with guidance for use. PCR Part B
2018-03 Institut Bauen und Umwelt e.V. (IBU), Requirements on the
EPD for fittings and showers. Version 1.1, Berlin, 03/2022
DIN EN ISO 50001
DIN EN ISO 50001:2018: Energy management systems — Thünen Institute
Requirements with guidance for use. 2018-08 Diestel, Sylvia / Weimar, Holger: Der Kohlenstoffgehalt in Holz-
und Papierprodukten - Herleitung und Umrechnungsfaktoren.
Further References Thünen Working Paper 38. Johann Heinrich von Thünen-
Institut. Hamburg,
9 Environmental Product Declaration - Hansgrohe Group - Shower Sets Standard
Publisher
Institut Bauen und Umwelt e.V. +49 (0)30 3087748- 0
Hegelplatz 1 info@ibu-epd.com
10117 Berlin www.ibu-epd.com
Germany
Programme holder
Institut Bauen und Umwelt e.V. +49 (0)30 3087748- 0
Hegelplatz 1 info@ibu-epd.com
10117 Berlin www.ibu-epd.com
Germany
Author of the Life Cycle Assessment
brands & values GmbH +49 421 70 90 84 33
Hollerallee 14A info@brandsandvalues.com
28209 Bremen www.brandsandvalues.com
Germany
Owner of the Declaration
Hansgrohe Group +49 7836 51-0
Auestr. 5-9 info@hansgrohe-group.com
77761 Schiltach www.hansgrohe-group.com
Germany
10 Environmental Product Declaration - Hansgrohe Group - Shower Sets Standard
