ENVIRONMENTAL PRODUCT DECLARATION
as per ISO 14025 and EN 15804+A2
Owner of the Declaration Etex Building Performance International
Programme holder Institut Bauen und Umwelt e.V. (IBU)
Publisher Institut Bauen und Umwelt e.V. (IBU)
Declaration number EPD-ETE-20200284-IBC1-EN
Issue date 01.04.2021
Valid to 31.03.2026
Duripanel A2
Etex Germany Exteriors GmbH
www.ibu-epd.com | https://epd-online.com
Umwelt Produktdeklaration Name des Herstellers – Name des Produkts
1. General Information
Etex Germany Exteriors GmbH Duripanel A2
Programme holder Owner of the declaration
IBU – Institut Bauen und Umwelt e.V. Etex Building Performance International
Panoramastr. 1 500 rue Marcel Demonque
10178 Berlin 84915 Avignon Cedex 9
Germany FRANCE
Declaration number Declared product / declared unit
EPD-ETE-20200284-IBC1-EN 1 m² Duripanel A2 with thickness 19mm.
This declaration is based on the product Scope:
category rules:
Wood cement - Mineral-bonded wooden composites, The life cycle assessment is based on production data
01.2019 of Duripanel A2 of the year 2018 at the production site
(PCR checked and approved by the SVR) of Etex Germany Exteriors GmbH in Beckum,
Germany.
Issue date The results of the life cycle assessment provided in this
01.04.2021 EPD are based on a thickness of 19mm and are
globally valid.
Valid to The LCA results for additional thicknesses are
declared in an annexe to this EPD.
31.03.2026
The owner of the declaration shall be liable for the
underlying information and evidence; the IBU shall not
be liable with respect to manufacturer information, life
cycle assessment data and evidences.
The EPD was created according to the specifications
of EN 15804+A2. In the following, the standard will be
simplified as EN 15804.
Verification
The standard EN 15804 serves as the core PCR
Independent verification of the declaration and data
according to ISO 14025:2010
Dipl. Ing. Hans Peters internally x externally
(chairman of Institut Bauen und Umwelt e.V.)
Dr. Alexander Röder Mr Carl-Otto Neven
(Managing Director Institut Bauen und Umwelt e.V.)) (Independent verifier)
2. Product
2.1 Information about the enterprise
Etex is an international building materials specialist For the placing on the market of the product in the
with headquarters in Belgium since 1905. The Etex European Union/European Free Trade Association
group operates 101 production sites in 42 countries (EU/EFTA) (with the exception of Switzerland)
and employs over 13 200 people worldwide. Regulation (EU) No. 305/2011 (CPR) applies. The
Duripanel is produced at the production site of Etex construction product is covered by the harmonized
Germany Exteriors GmbH. declaration of performance No. Si-
DOP/Duripanel_A2/v01.10.2020 taking into
2.2 Product description/Product definition consideration EN 13986: 2015, Wood-based panels for
Duripanel A2 is a three-layer cement-bonded use in construction - Characteristics, evaluation of
particleboard according to EN 634-1 and -2 for internal conformity and marking and the CE-marking.
and external construction applications. It mainly For the application and use the respective national
consists of the natural raw material wood particles and provisions apply.
cement.
It is being produced in different thicknesses between 2.3 Application
10 and 32 mm. It is available in an unsanded smooth The Duripanel A2 base panel with straight edges can
or sanded surface, with smooth trimmed edges or with be used for high-quality interior finishing, roof
tongue and groove. The surface colour is mainly being formwork, timber construction and container
characterized by the fine wood particles in the outside construction with increased fire protection
layers. requirements for non-combustible building materials.
2 Environmental Product Declaration Etex Germany Exteriors GmbH – Duripanel A2
The Duripanel A2 installation panel with tongue and - 55-75% Portland cement
groove can be used for load-bearing formwork and dry - 5-15% spruce wood (Atro)
subfloors with high compressive strength and chair - 5-15% perlite
castor suitability (screw-fixing) with increased fire
protection requirements for non-flammable building By using cement as a binder, no binder related
materials. isocyanates, synthetic resin or formaldehyde are being
added. No wood protection agents are being used.
2.4 Technical Data This article contains substances listed in the candidate
list (date: 19.01.2021) exceeding 0.1 percentage by
The constructional data shown in the table are valid for mass: no.
all thicknesses and surfaces (sanded/unsanded), This article contains other carcinogenic, mutagenic,
unless where indicated otherwise. reprotoxic (CMR) substances in categories 1A or 1B
which are not on the candidate list, exceeding 0.1
Constructional data percentage by mass: no.
Name Value Unit Biocide products were added to this construction
Raw density acc. to EN 634- product or it has been treated with biocide products
≥ 1000 kg/m³
2:2007; EN 13986:2004+A1:2015 (this then concerns a treated product as defined by the
Grammage (19 mm) 26.1 kg/m2 (EU) Ordinance on Biocide Products No. 528/2012):
Bending strength (longitudinal) ≥ 9 N/mm2 no.
Bending strength (transverse) ≥ 9 N/mm2
E-module (longitudinal) ≥ 4500 N/mm2 2.7 Manufacture
E-module (transverse) ≥ 4500 N/mm2 The production of large-format panels from wood
Tensile strength rectangular cement takes place according to a largely automated,
(internal bond) ≥ 0.5 N/mm2 semi-dry spreading process in which no excess water
is produced. In a mechanical mixer, the litter mixture of
Thermal conductivity λ acc. to DIN
0.23 W/(mK) wood chips, cement, recycled material from trimming
EN 13986:2015
waste, auxiliary materials and water is processed. The
sanded: 64
material is evenly distributed on carrier plates via a
(moist);
Water vapour diffusion resistance mechanical throw sifting system. Excess material at
143 (dry)
factor µ acc. to DIN EN ISO - the edges is returned directly to the spreader. The
unsanded:
12572:2001 scattered material is pressed, stored in a climatic
90 (moist);
chamber for setting (heat exchanger, steam generation
135 (dry)
via natural gas), the hardened sheets restacked,
Moisture content at 23 °C, 80%
9 Vol. % trimmed and temporarily stored for 28 days. The
acc. to DIN EN ISO 12571:2000
panels are then dried in a circulating air oven to the
Coefficient of thermal expansion
11 10-6K-1 moisture content required for delivery.
αt
Swelling in thickness 24h acc. to
≤ 1,5 % The quality management system of the company and
EN 634-2: 2007
the production facility are certified according to ISO
Sound absorption coefficient α 10 at 250-
9001:2015.
(only with reference to the 500Hz / 30
%
corresponding component design) at 1000-
2.8 Environment and health during
acc. to EN 13986:2004+A1:2015 2000Hz
manufacturing
During the entire manufacturing process, no health and
safety measures are required beyond the legally
For more detailed info on product characteristics
stipulated occupational health and safety measures for
please refer to the latest DOP.
commercial enterprises.
The performance data of the product is in accordance
Air: Any dust produced is collected in filter systems
with the declaration of performance with respect to its
and partially recycled. The emissions are well below
essential characteristics according to the standards
the limit values of TA Luft.
mentioned in the headline in the table for
constructional data.
Water/Soil: The water resulting from production and
plant cleaning is mechanically clarified in wastewater
treatment plants on the factory premises and reused in
2.5 Delivery status
the production process.
Duripanel A2 basic panels are available in two sizes
1250 x 2600 mm or 1250 x 3100 mm.
Noise: Noise emissions from production plants to the
The panels are delivered sanded and unsanded in
environment are below the permissible limits.
various thicknesses:
10, 13, 16, 19, 22, 25, 28, 32 mm.
The environmental management system of the
company and the production facility are certified ISO
Duripanel A2 installation panels are available in sizes
14001:2015.
1250 x 625 mm. The panels are delivered sanded on
both sides in thicknesses 19 and 25 mm.
2.9 Product processing/Installation
The processing of Duripanel can include the following
processes, for example: sawing, drilling, grinding.
2.6 Base materials/Ancillary materials
Under certain conditions Duripanel can be milled.
The main raw materials used are (in weight
percentages; dry):
3 Environmental Product Declaration Etex Germany Exteriors GmbH – Duripanel A2
Fixing the boards will require appropriate means, according to Bewertungssystem Nachhaltiges
which will depend upon the application and bearing Bauen (BNB)" is indicated to be >50 years.
structure. Boards can be installed using screws or Over the service life, free lime in the cement reacts
glues. Under certain conditions, the boards can be with carbon dioxide in the air to form calcium
fixed using clamps. carbonate (carbonation). There will be no verifiable
When selecting structurally necessary additional influences on ageing when the products are applied in
products, care must be taken that these do not accordance with the generally accepted rules of
adversely affect the described properties of the technology.
environmental compatibility of the construction
products mentioned.
2.14 Extraordinary effects
The local regulations for the workers’ health and safety
and the environment apply (e.g. trade associations or Fire
ordinance on hazardous substances). Also, when The Duripanel A2 boards have a fire classification
processing the above-mentioned products, the usual according to EN 13501-1 as given in the table below.
occupational health and safety measures must be
observed in accordance with the manufacturer's Fire protection
instructions. It should be noted that dust produced Name Value
during processing can react alkaline (pH value: approx. Building material class - base panel A2
12). The machining tools and equipment used at the Smoke gas development - base panel s1
workplace should be such that the relevant dust limits Burning droplets - base panel d0
are observed. Building material class - installation panel A2
For example, in Germany the general dust limit value Smoke gas development - installation panel s1
is given in the directive TRGS 900. According to Burning droplets - installlation panel -
current knowledge, water, air and soil cannot be
endangered if wood cement is processed as intended. Water
No ingredients that could be hazardous to water are
2.10 Packaging washed out (see also item Evidence: Eluate analysis).
PE shrink films, paper, wooden pallets and steel The pH value is basic (pH ≥ 12).
strapping are used as packaging materials. The
wooden pallets used are one-way pallets. Mechanical destruction
Extraordinary effects related to a mechanical
destruction (e.g. emissions) are not known.
2.11 Condition of use
Duripanel building boards are resistant to the effects of 2.15 Re-use phase
moisture and are not physically affected when used in Several possibilities exist for the boards after the end-
humid or wet conditions. Some performance of-life of the application in which they were used.
characteristics are affected by moisture content. The
panels do not promote mould growth and are resistant In undamaged form, the dismantled products can be
to attacks by insects or vermin. used again in accordance with their original purpose
or, for example, be reused as foundation wall
Setting (hydration) of the cement-water mixture protection.
produces hardened cement paste (calcium silicate If not contaminated with other building construction
hydrates) with embedded wood chips, ground material, the boards can be ground up again and
production waste and auxiliary materials, with the reused as an additive in the production of wood
proportions indicated in the item 2.5 "Base materials". cement (material recycling).
Over the period of use, free lime from the cement
reacts with carbon dioxide from the air to form calcium Furthermore, the products referred to could be used as
carbonate (carbonation). filler and bulk material in civil engineering, road
construction or e.g. for noise barriers (material
Wood cement contains approx. 9-11 % water recycling).
(equilibrium moisture) which can vary with the
environmental conditions. In addition, material and energetic recycling in the
cement plant is possible.
2.12 Environment and health during use
Duripanel A2 is chemically inert. When the product is 2.16 Disposal
used as designed, the current state of knowledge For the consideration of possible disposal channels,
indicates that hazards to water, air and soil cannot the following disposal stages are proposed:
arise.
A) Production waste (before use)
The ingredients of the construction product are firmly B) Waste generated before use
bound in the state of use. Dust emissions will not occur a) at a finishing company that cuts panels to size
unless the boards are machined with abrasive tools. In b) during installation on the building site
case of contact (skin, eye, mouth contact), it should be C) Waste after use, when a building is demolished or
noted that hardened cement paste reacts slightly when structural changes are made during the use
alkaline in combination with moisture. phase of the building.
2.13 Reference service life Disposal channels at stage A)
The service life according to the “Bundesinstitut für If the wood cement products are separated by type in
Bau-, Stadt- und Raumforschung“ (BBSR) table the factory, they can be ground again and reused as
“Service lives of components for life cycle assessment
4 Environmental Product Declaration Etex Germany Exteriors GmbH – Duripanel A2
an additive in the production of wood cement (material As the landfill classes are being defined differently in
recycling). This shall be preferred. the member states, the landfill class of the respective
Thermal treatment in residual waste treatment plants country applies.
and cement works can be considered.
The lowest priority route may be landfill. The following waste codes are suggested:
Disposal channel A) 10 13 11 (wastes from cement-
Disposal channels at stage B) and C) based composite materials other than those mentioned
a) At collection: keeping cement-bonded particleboard in 10 13 09 and 10 13 10).
separate from wood waste as well as from other Disposal channels B) and C) 17 09 04 (mixed
mineral wastes construction and demolition wastes other than those
b) Thermal treatment and/or energy recovery mentioned in 17 09 01, 17 09 02 and 17 09 03).
c) Landfill
2.17 Further information
As for disposal facilities, depending on the composition Further information can be found on the homepage
and quantity of waste, thermal residual waste https://www.siniat.com/.
treatment plants and cement works can be considered.
3. LCA: Calculation rules
3.1 Declared Unit  efforts for the use of the product,
The functional unit declared in this EPD is 1m² of maintenance and operational efforts
Duripanel A2 with a thickness of 19mm (abbreviated
 modules B3, B4, B5 are declared as MNR
as 1m²19mm).
(module not relevant) according to the IBU
In an annexe to this EPD, the LCA results for the other
existing thicknesses are declared. requirement. These modules are defined on
building level in general.
Declared unit
Name Value Unit
End-of-life stage (C1-C4):
Declared unit 1 m²
Two end-of-life scenarios were considered:
Gross density used in calculations
1373 kg/m3
based on 2018 average data
1) Scenario 1: 100% recycling in cement plant.
Grammage 26.1 kg/m2 Due to the wood content of Duripanel B1, the shredded
Conversion factor to 1 kg (kg/m²) 26.1 - product can reduce the use of energy in the cement
Layer thickness 0,019 m plant during cement clinker production.
Simultaneously, the other raw material components in
the wood cement boards help to reduce the use of
virgin raw materials in the cement plant. Energy and
3.2 System boundary material credits were assigned using the substitution
Type of the EPD: cradle to grave. approach. The resulting credits from energy recovery
The following life cycle stages and modules are and material recycling are assigned to module D.
included:
2) Scenario 2: 100% landfilling.
Production stage (A1-A3):
 manufacturing of pre products and For both scenarios, the following processes were
transportation to the manufacturing site included:
 energy consumption during production  energy consumption for deconstruction and
 recycling and disposal of production wastes demolition
 production of packaging  transportation to disposal
 waste processing and recycling or landfilling
of product
Construction stage (A4-A5):
 transportation of product to the construction
site Loads and benefits beyond system boundary (D):
 energy consumption during the installation of  loads and benefits from recycling/landfilling of
products production waste, packaging, installation
losses and product waste.
 production of fixing material
 disposal of installation wastes including
emissions of biogenic CO2 from the wood
content
3.3 Estimates and assumptions
 incineration/recycling of packaging materials
Most of the input and output influences of the Life
(potential benefits from energy substitution
Cycle Inventory Analyses could be depicted using
within the incineration process are declared in corresponding data from the GaBi database.
module D) including emissions of biogenic There were no data records available for the wooden
CO2 from renewable packaging materials pallets, they were approximated using the solid
construction timber dataset. For well water, a worst-
case scenario dataset “tap water from groundwater”
Use stage (B1-B7):
was used. For the Duripanel product waste sent to
5 Environmental Product Declaration Etex Germany Exteriors GmbH – Duripanel A2
landfill, a combination of an inert waste dataset and a
municipal solid waste dataset was used in a ratio to 3.8 Allocation
match the calorific value of the Duripanel B1 waste. Allocation in background data
Bluewater consumption is taken into consideration in Specific information on allocation within the
the background data system. Water which is background data is given in the GaBi documentation.
embedded in the product, as well as water which is Allocation in foreground data
evaporated from the product during production, is The production process does not deliver any co-
included in the calculations. products. In module A1-A3, specific raw material,
water and transport data were available.
3.4 Cut-off criteria Thermal energy used at plant level in a cogeneration
All available data from production processes were unit could not be directly allocated to the product and
considered, i.e., all pre-products used, thermal energy was allocated via recalculation based on consumed
and electric power consumption as well as waste amounts of electricity and steam.
management processes using the best available life Allocation for waste materials
cycle inventory (LCI) datasets. This includes input The environmental burden of waste treatment of the
flows with a contribution of less than 1% of mass or installation loss and the incineration of packaging is
energy. assigned to the system in A5. The resulting credits for
Production of capital equipment, facilities and thermal and electrical energy are declared in module
infrastructure required for manufacture are outside the D.
scope of this assessment. The environmental burdens of the product at end-of-life
scenarios are assigned to C3 and C4, the resulting
3.5 Background data credits for thermal and electrical energy are declared in
The GaBi ts software was used to model the product module D.
life cycle. The background data were sourced from the
GaBi database. 3.9 Comparability
Basically, a comparison or an evaluation of EPD data
3.6 Data quality is only possible if all the data sets to be compared
This study is mainly based on primary data collected were created according to EN 15804 and the building
directly from the manufacturing site and therefore data context, respectively the product-specific
quality can be assumed to be very good. characteristics of performance, are taken into account.
Background data are from the GaBi database, last
update was in 2020. GaBi database version 2020.1, SP40 serves as
background database for the calculation of the life
3.7 Period under review cycle assessment..
Data for the entire production period of 2018 were
collected and used for this EPD.
4. LCA: Scenarios and additional technical information
Characteristic product properties
Information on biogenic Carbon Use or application of the installed product (B1) see
section 2.12 "Use"
No efforts and releases of substances occur during the
Information on describing the biogenic Carbon normal (i.e. anticipated) use phase
Content at factory gate Name Value Unit
Name Value Unit
Biogenic Carbon Content in Maintenance (B2)
1.31 kg C
product No efforts occur during maintenance.
Biogenic Carbon Content in Name Value Unit
0.22 kg C
accompanying packaging Water consumption 0 m3
Auxiliary 0 kg
Other resources 0 kg
Electricity consumption 0 kWh
Other energy carriers 0 MJ
Transport to the building site (A4) Material loss 0 kg
Name Value Unit
Transport distance 300 km
Capacity utilisation (including empty
61 %
runs)
Gross density of products transported 1373 kg/m3
Installation into the building (A5)
Name Value Unit
Auxiliary galvanized steel screws 0.12 kg
Electricity consumption 0.075 kWh
Material loss 2.61 kg
Dust in the air 0 kg
VOC in the air 0 kg
6 Environmental Product Declaration Etex Germany Exteriors GmbH – Duripanel A2
Steel strip packaging 7 g
EoL Recycling (scenario 1) 26.22 kg
EoL Recycling (scenario 2) 0.12 kg
Reference service life
Name Value Unit
Reference service life (according
- a
to ISO 15686-1, -2, -7 and -8)
Life Span (according to BBSR) >=50 a
Life Span according to the
- a
manufacturer
Declared product properties (at
- -
the gate) and finishes
Design application parameters (if
instructed by the manufacturer),
including the references to the - -
appropriate practices and
application codes
An assumed quality of work, when
installed in accordance with the - -
manufacturer’s instructions
Outdoor environment, (for outdoor
applications), e.g. weathering,
pollutants, UV and wind exposure, - -
building orientation, shading,
temperature
Indoor environment (for indoor
applications), e.g. temperature, - -
moisture, chemical exposure
Usage conditions, e.g. frequency
- -
of use, mechanical exposure
Maintenance e.g. required
frequency, type and quality and - -
replacement of components
Operational energy use (B6) and Operational water
use (B7)
No efforts occur in modules B6 and B7.
Name Value Unit
Water consumption 0 m3
Electricity consumption 0 kWh
Other energy carriers 0 MJ
Equipment output 0 kW
End-of-life (C1-C4)
Two end-of-life scenarios are considered :
- scenario 1: 100% recycling in cement plant
- scenario 2: 100% landfill
Name Value Unit
Collected as mixed construction
26.22 kg
waste
Recycling (scenario 1) 26.22 kg
Recycling (scenario 2) 0.12 kg
Landfilling (scenario 1) 0 kg
Landfilling (scenario 2) 26.1 kg
Reuse, recovery and/or recycling potentials (D),
relevant scenario information
Possible benefits from the recycling of production
waste and installation losses were considered. Also
benefits from the incineration of packaging were
considered. Additionally, benefits from the recycling of
the product at the end-of-life was taken into account
according to the selected scenario.
Name Value Unit
Recycled production waste 1.43 kg
Recycled installation losses 0.913 kg
PE packaging 14 g
Wood packaging 546 g
Paper packaging 3 g
7 Environmental Product Declaration Etex Germany Exteriors GmbH – Duripanel A2
5. LCA: Results
Disclaimer – for the indicator EF-freshwater, this indicator (the kg PO4 eq.) has been calculated as “kg P eq.” as
required in the characterization model EC-JRC : EF 3.0; http://eplca.jrc.ec.europa.eu/LCDN/developerEF.xhtml.
The characterization factors are available both in ILCD structure and as Excel file and they are identified by the
name EN_15804.
DESCRIPTION OF THE SYSTEM BOUNDARY (X = INCLUDED IN LCA; ND = MODULE OR INDICATOR NOT
DECLARED; MNR = MODULE NOT RELEVANT)
BENEFITS AND
CONSTRUCTI LOADS
PRODUCT STAGE ON PROCESS USE STAGE END OF LIFE STAGE BEYOND THE
STAGE SYSTEM
BOUNDARIES
8 Environmental Product Declaration Etex Germany Exteriors GmbH – Duripanel A2
lairetam
waR
ylppus tropsnarT
gnirutcafunaM
eht
morf
tropsnarT
etis
eht
ot
etag
ylbmessA esU
ecnanetniaM
riapeR
tnemecalpeR tnemhsibrufeR
ygrene
lanoitarepO esu
retaw
lanoitarepO esu
noitcurtsnoc-eD
noitilomed tropsnarT
gnissecorp
etsaW
lasopsiD -esueR -yrevoceR -gnilcyceR laitnetop
A1 A2 A3 A4 A5 B1 B2 B3 B4 B5 B6 B7 C1 C2 C3 C4 D
X X X X X X X MNR MNR MNR X X X X X X X
RESULTS OF THE LCA - ENVIRONMENTAL IMPACT according to EN 15804+A2: 1 m²19mm Duripanel A2
Core Indicator Unit A1-A3 A4 A5 B1 B2 B6 B7 C1 C2 C3/1 C3/2 C4/1 C4/2 D/1 D/2
- -
1.73E+ 4.17E+ 0.00E+ 0.00E+ 0.00E+ 0.00E+ 1.47E+ 0.00E+ 0.00E+ 1.02E+
GWP-total [kg CO2-Eq.]
1
6.12E-1
0 0 0 0 0
3.03E-21.00E-1
0 0 0 1
3.99E+ 1.04E+
0 0
- -
2.25E+ 2.82E+ 0.00E+ 0.00E+ 0.00E+ 0.00E+ 1.46E+ 0.00E+ 0.00E+ 1.32E+
GWP-fossil [kg CO2-Eq.]
1
6.08E-1
0 0 0 0 0
3.02E-29.93E-2
0 0 0 0
3.99E+ 1.04E+
0 0
-
-1.02E- 1.35E+ 0.00E+ 0.00E+ 0.00E+ 0.00E+ -1.67E- 0.00E+ 0.00E+ 8.88E+ -2.26E- -1.96E-
GWP-biogenic [kg CO2-Eq.] 5.20E+
3 0 0 0 0 0
1.01E-4
4
4.86E-3
0 0 0 3 3
0
0.00E+ 0.00E+ 0.00E+ 0.00E+ 0.00E+ 0.00E+ -9.74E- -7.70E-
GWP-luluc [kg CO2-Eq.] 6.97E-34.92E-31.14E-3
0 0 0 0
4.38E-58.04E-42.11E-3
0 0
1.21E-3
4 4
8.17E- 1.12E- 1.15E- 0.00E+ 0.00E+ 0.00E+ 0.00E+ 6.64E- 1.82E- 3.21E- 0.00E+ 0.00E+ 2.09E- -5.22E- -1.04E-
ODP [kg CFC11-Eq.]
14 16 14 0 0 0 0 16 17 14 0 0 15 15 14
0.00E+ 0.00E+ 0.00E+ 0.00E+ 0.00E+ 0.00E+ -4.09E- -1.86E-
AP [mol H+-Eq.] 2.66E-27.02E-44.18E-3 6.66E-51.15E-43.22E-3 4.42E-3
0 0 0 0 0 0 3 3
0.00E+ 0.00E+ 0.00E+ 0.00E+ 0.00E+ 0.00E+ -1.59E- -1.43E-
EP-freshwater [kg PO4-Eq.] 3.75E-51.85E-62.37E-5
0 0 0 0
8.06E-83.03E-73.90E-6
0 0
1.92E-4
6 6
0.00E+ 0.00E+ 0.00E+ 0.00E+ 0.00E+ 0.00E+ -1.46E- -4.54E-
EP-marine [kg N-Eq.] 8.86E-32.16E-41.41E-3 1.48E-53.53E-57.15E-4 2.65E-3
0 0 0 0 0 0 3 4
0.00E+ 0.00E+ 0.00E+ 0.00E+ 0.00E+ 0.00E+ -1.61E- -4.86E-
EP-terrestrial [mol N-Eq.] 9.64E-22.56E-31.40E-2 1.56E-44.19E-47.51E-3 1.44E-2
0 0 0 0 0 0 2 3
0.00E+ 0.00E+ 0.00E+ 0.00E+ 0.00E+ 0.00E+ -4.38E- -1.33E-
POCP [kg NMVOC-Eq.]2.70E-25.82E-44.16E-3 4.06E-59.51E-51.96E-3 6.67E-3
0 0 0 0 0 0 3 3
0.00E+ 0.00E+ 0.00E+ 0.00E+ 0.00E+ 0.00E+ -2.63E- -1.63E-
ADPE [kg Sb-Eq.] 9.88E-74.91E-82.19E-5 8.74E-98.03E-94.22E-7 5.76E-8
0 0 0 0 0 0 7 7
- -
1.46E+ 8.11E+ 1.98E+ 0.00E+ 0.00E+ 0.00E+ 0.00E+ 1.33E+ 2.56E+ 0.00E+ 0.00E+ 1.07E+
ADPF [MJ] 5.31E-1 6.36E+ 1.60E+
2 0 1 0 0 0 0 0 1 0 0 1
1 1
[m³ world-Eq 0.00E+ 0.00E+ 0.00E+ 0.00E+ 0.00E+ 0.00E+ -4.55E- -1.07E-
WDP 3.83E-15.93E-31.65E-1 6.58E-39.68E-43.18E-1 6.02E-2
deprived] 0 0 0 0 0 0 2 1
GWP = Global warming potential; ODP = Depletion potential of the stratospheric ozone layer; AP = Acidification potential of land and water; EP =
Caption Eutrophication potential; POCP = Formation potential of tropospheric ozone photochemical oxidants; ADPE = Abiotic depletion potential for non-
fossil resources; ADPF = Abiotic depletion potential for fossil resources; WDP = Water (user) deprivation potential
RESULTS OF THE LCA - INDICATORS TO DESCRIBE RESOURCE USE according to EN 15804+A2: 1
m²19mm Duripanel A2
Indicator Unit A1-A3 A4 A5 B1 B2 B6 B7 C1 C2 C3/1 C3/2 C4/1 C4/2 D/1 D/2
PERE [MJ] 2.67E+1 4.69E-1 1.76E+10.00E+00.00E+00.00E+00.00E+0 2.35E-1 7.66E-2 5.71E+10.00E+00.00E+04.66E+1-1.96E+0-3.81E+0
PERM [MJ] 5.42E+10.00E+0-8.49E+00.00E+00.00E+00.00E+00.00E+00.00E+00.00E+0-4.57E+10.00E+00.00E+0-4.57E+10.00E+00.00E+0
PERT [MJ] 8.09E+1 4.69E-1 9.11E+00.00E+00.00E+00.00E+00.00E+0 2.35E-1 7.66E-2 1.14E+10.00E+00.00E+0 9.54E-1-1.96E+0-3.81E+0
PENRE [MJ] 1.46E+28.14E+02.04E+10.00E+00.00E+00.00E+00.00E+0 5.31E-1 1.33E+02.56E+10.00E+00.00E+01.07E+1-6.37E+1-1.60E+1
PENRM [MJ] 5.62E-1 0.00E+0-5.62E-10.00E+00.00E+00.00E+00.00E+00.00E+00.00E+00.00E+00.00E+00.00E+00.00E+00.00E+00.00E+0
PENRT [MJ] 1.46E+28.14E+01.98E+10.00E+00.00E+00.00E+00.00E+0 5.31E-1 1.33E+02.56E+10.00E+00.00E+01.07E+1-6.37E+1-1.60E+1
SM [kg] 0.00E+00.00E+0 1.49E-1 0.00E+00.00E+00.00E+00.00E+00.00E+00.00E+00.00E+00.00E+00.00E+00.00E+00.00E+00.00E+0
RSF [MJ] 0.00E+00.00E+00.00E+00.00E+00.00E+00.00E+00.00E+00.00E+00.00E+00.00E+00.00E+00.00E+00.00E+00.00E+00.00E+0
NRSF [MJ] 0.00E+00.00E+00.00E+00.00E+00.00E+00.00E+00.00E+00.00E+00.00E+00.00E+00.00E+00.00E+00.00E+00.00E+00.00E+0
FW [m³] 1.80E-2 5.46E-4 5.52E-3 0.00E+00.00E+00.00E+00.00E+0 2.72E-4 8.93E-5 1.31E-2 0.00E+00.00E+0 1.85E-3-2.35E-3-4.68E-3
PERE = Use of renewable primary energy excluding renewable primary energy resources used as raw materials; PERM = Use of
renewable primary energy resources used as raw materials; PERT = Total use of renewable primary energy resources; PENRE = Use of
non-renewable primary energy excluding non-renewable primary energy resources used as raw materials; PENRM = Use of non-
Caption
renewable primary energy resources used as raw materials; PENRT = Total use of non-renewable primary energy resources; SM = Use
of secondary material; RSF = Use of renewable secondary fuels; NRSF = Use of non-renewable secondary fuels; FW = Use of net fresh
water
RESULTS OF THE LCA – WASTE CATEGORIES AND OUTPUT FLOWS according to EN 15804+A2:
1 m²19mm Duripanel A2
Indicator Unit A1-A3 A4 A5 B1 B2 B6 B7 C1 C2 C3/1 C3/2 C4/1 C4/2 D/1 D/2
HWD [kg] 3.45E-7 3.76E-7 4.56E-8 0.00E+00.00E+00.00E+00.00E+02.20E-106.15E-8 1.06E-8 0.00E+00.00E+0 8.22E-8-5.26E-8-8.50E-9
NHWD [kg] 3.79E+0 1.29E-3 2.82E+00.00E+00.00E+00.00E+00.00E+0 3.77E-4 2.11E-4 1.82E-2 0.00E+00.00E+02.43E+1-1.86E-2-1.01E-2
RWD [kg] 1.79E-3 1.50E-5 3.92E-4 0.00E+00.00E+00.00E+00.00E+0 8.06E-5 2.45E-6 3.89E-3 0.00E+00.00E+0 1.26E-4-5.75E-4-1.32E-3
CRU [kg] 0.00E+00.00E+00.00E+00.00E+00.00E+00.00E+00.00E+00.00E+00.00E+00.00E+00.00E+00.00E+00.00E+00.00E+00.00E+0
MFR [kg] 1.19E+00.00E+0 1.26E-1 0.00E+00.00E+00.00E+00.00E+00.00E+00.00E+02.19E+1 9.98E-2 0.00E+00.00E+00.00E+00.00E+0
MER [kg] 2.36E-1 0.00E+0 2.36E-2 0.00E+00.00E+00.00E+00.00E+00.00E+00.00E+04.30E+00.00E+00.00E+02.71E+00.00E+00.00E+0
EEE [MJ] 2.81E-3 0.00E+01.79E+00.00E+00.00E+00.00E+00.00E+00.00E+00.00E+00.00E+00.00E+00.00E+00.00E+00.00E+00.00E+0
EET [MJ] 6.48E-3 0.00E+02.76E+00.00E+00.00E+00.00E+00.00E+00.00E+00.00E+00.00E+00.00E+00.00E+00.00E+00.00E+00.00E+0
HWD = Hazardous waste disposed; NHWD = Non-hazardous waste disposed; RWD = Radioactive waste disposed; CRU = Components
Caption for re-use; MFR = Materials for recycling; MER = Materials for energy recovery; EEE = Exported electrical energy; EEE = Exported
thermal energy
RESULTS OF THE LCA – additional impact categories according to EN 15804+A2-optional:
1 m²19mm Duripanel A2
Indicator Unit A1-A3 A4 A5 B1 B2 B6 B7 C1 C2 C3/1 C3/2 C4/1 C4/2 D/1 D/2
[Disease 5.59E- 7.61E-
PM 5.28E-7 4.66E-9 6.85E-80.00E+00.00E+00.00E+00.00E+0 2.70E-80.00E+00.00E+04.88E-8-2.21E-7-2.72E-8
Incidence] 10 10
[kBq U235-
IR 1.79E-1 2.21E-3 4.45E-20.00E+00.00E+00.00E+00.00E+01.32E-2 3.62E-4 6.38E-10.00E+00.00E+01.63E-2-9.20E-2-2.19E-1
Eq.]
- -
ETP-fw [CTUe] 6.84E+16.07E+09.40E+00.00E+00.00E+00.00E+00.00E+02.27E-1 9.91E-11.10E+10.00E+00.00E+01.25E+1
3.28E+04.14E+0
1.25E- 6.63E- 6.27E- 2.05E- 3.03E- 6.66E- -7.46E- -4.18E-
HTP-c [CTUh] 2.19E-9 0.00E+00.00E+00.00E+00.00E+0 0.00E+00.00E+0
10 10 12 11 10 10 10 10
2.31E-
HTP-nc [CTUh] 1.70E-7 6.40E-9 2.87E-80.00E+00.00E+00.00E+00.00E+0 1.05E-9 1.12E-80.00E+00.00E+06.82E-8-2.07E-8-6.69E-9
10
- -
SQP [-] 5.88E+22.85E+05.98E+10.00E+00.00E+00.00E+00.00E+01.69E-1 4.65E-18.17E+00.00E+00.00E+01.26E+0
2.08E+02.77E+0
PM = Potential incidence of disease due to PM emissions; IR = Potential Human exposure efficiency relative to U235; ETP-fw = Potential
Caption comparative Toxic Unit for ecosystems; HTP-c = Potential comparative Toxic Unit for humans (cancerogenic); HTP-nc = Potential
comparative Toxic Unit for humans (not cancerogenic); SQP = Potential soil quality index
Disclaimer 1 – for the indicator IRP : this impact category deals mainly with the eventual impact of low dose
ionizing radiation on human health of the nuclear fuel cycle. It does not consider effects due to possible nuclear
accidents, occupational exposure nor due to radioactive waste disposal in underground facilities. Potential
ionizing radiation from the soil, from radon and from some construction materials is also not measured by this
indicator.
Disclaimer 2 – for the indicators ADPE, ADPF, WDP, ETP-fw, HTP-c, HTP-nc, SQP : the results of this
environmental impact indicator shall be used with care as the uncertainties on these results are high or as there is
limited experienced with the indicator.
6. LCA: Interpretation
Looking at the overall life cycle for the scenario 1 contribution (>50%) in GWP biogenic and EP
(recycling), for most of the impact categories (except freshwater.
for GWP-luluc, ADP-minerals&metals and WDP), the
manufacturing of Duripanel A2 contributes to the Within A1-A3, the pre-chains of the raw material have
largest share (>50%) to the environmental the most important impact in all impact categories
performance. except for GWP total/ ADP-fossil and EP-freshwater,
followed by the energy consumption for the
The C3 phase has only minor impacts, except in the production. Transport to site (A2) has a negligible
category ODP and WDP relevant influences can be influence (<2.5%) on the overall LCA results (except
seen, linked to the electricity use for shredding the for GWP-luluc where it has little influence (<10%)).
waste material.
The LCA for Duripanel A2 is in module A1 almost fully
Looking at the overall life cycle for the scenario 2 determined by the pre-chains of the cement in all
(landfill) in most of the impact categories (except for impact categories except in the GWP-total and
GWP-biogenic and -luluc, EP freshwater and ADP- biogenic where the wood has high impact and in WDP
minerals&metals), the manufacturing of Duripanel A2 where the water consumed in the Duripanel process
contributes to the largest share (>50%) to the has a very important contribution.
environmental performance.
For the GWP-total and the GWP-biogenic, next to the
production phase, the main impacts occur in module
C4 linked to the EOL landfilling of the waste and re-
emission of organic carbon dioxide linked to it.
For the EP-freshwater, the production waste sent to
landfill in C4 is the main contributor.
The C4 phase has very important impacts (>25%) in
the category GWP total and and the most important
9 Environmental Product Declaration Etex Germany Exteriors GmbH – Duripanel A2
7. Requisite evidence
Cu Cupper <0.005 mg/l
7.1 Testing pretreatment of substances used Mo Molybdenum <0.005 mg/l
Measurements according to the Waste Wood Ni Nickel 0.0296 mg/l
Ordinance are not relevant as no waste wood is used Hg Mercury <0.2 mg/l
in the manufacture of Duripanel B1 wood cement Se Selenium <0.002 mg/l
products. Zn Zinc <0.0206 mg/l
7.2 Leaching 7.3 VOC emissions
Measurement in accordance with EN 71-3, University Measurements in line with the AgBB diagram; Eurofins
of Osnabrück, Institute of Chemistry, Osnabrück; Product Testing A/S, Galten, Denmark 09.09.2010.
03.02.2000
Results : the analysis results of the leaching of the AgBB overview of results (28 days [µg/m³])
examined boards showed that the limit values laid Name Value Unit
down in EN 71 were complied with. TVOC (C6 - C16) 36 μg/m3
Sum SVOC (C16 - C22) 19 μg/m3
Measurement in accordance with EN 12457-4, UCL R (dimensionless) 0.02 -
Umwelt Control Labor GmbH, Lünen; 23.07.2019 : VOC without NIK 5.8 μg/m3
Carcinogenic Substances <0.1 μg/m3
Name Value Unit AgBB overview of results (3 days [µg/m³])
Sb Antimony <0.001 mg/l
Name Value Unit
As Arsenic <0.001 mg/l
TVOC (C6 - C16) < μg/m3
Ba Barium 0.502 mg/l
Sum SVOC (C16 - C22) 0 - 0.5 μg/m3
Pb Lead 0.047 mg/l
VOC without NIK 23 μg/m3
Cd Cadmium <0.0003 mg/l
Carcinogenic Substances 0 - 0.1 μg/m3
Cr Chromium 0.0023 mg/l
8. References
Standards EN 15804
EN 15804:2012+A2:2019, Sustainability of
DIN EN 1995-1-1/NA construction works — Environmental Product
DIN EN 1995-1-1/NA:2013-08, National Annex – Declarations — Core rules for the product category of
Nationally determined parameters – Eurocode 5: construction products.
Design of timber structures – Part 1-1: General –
Common rules and rules for buildings. EN 1995-1-1
EN 1995-1-1:2004/A2:2014, Eurocode 5: Design of
DIN 4102-1 timber structures – Part 1-1: General – Common rules
DIN 4102-1:1998, Fire behaviour of building materials and rules for buildings.
and elements - Classification of building materials -
Requirements and testing. EN 634-1
EN 634-1:1995, Cement-bonded particleboards -
EN ISO 14025 Specifications - Part 1: General requirements.
DIN EN ISO 14025:2011-10, Environmental labels and
declarations — Type III environmental declarations — EN 634-2
Principles and procedures. EN 634-2:2007, Cement-bonded particleboards -
Specifications - Part 2: Requirements for OPC bonded
EN 12457-4 particleboards for use in dry, humid and external
EN 12457-4:2002, Characterisation of waste. conditions.
Leaching. Compliance test for leaching of granular
waste materials and sludges. One stage batch test at a EN 71-3
liquid to solid ratio of 10 l/kg for materials with particle EN 71-3:2019, Safety of toys - Part 3: Migration of
size below 10 mm (without or with size reduction). certain elements.
EN 13501-1 ISO 12571
EN 13501-1:2018, Fire classification of construction DIN EN ISO 1271:2000, Hygrothermal performance of
products and building elements - Part 1: Classification building materials and products — Determination of
using data from reaction to fire tests. hygroscopic sorption properties.
EN 13986 ISO 12572
DIN EN 13986:2015-06, Wood-based panels for use in DIN EN ISO 12572:2001, Hygrothermal performance
construction - Characteristics, evaluation of conformity of building materials and products - Determination of
and marking. water vapour transmission properties - Cup method
10 Environmental Product Declaration Etex Germany Exteriors GmbH – Duripanel A2
ISO 14025
DIN EN ISO 14025:2011-10, Environmental labels and IBU 2016
declarations — Type III environmental declarations — Institut Bauen und Umwelt e.V.: General Programme
Principles and procedures. Instructions for the Preparation of EPDs at the Institut
Bauen und Umwelt e.V. Version 1.1, Berlin: Institut
ISO 9001 Bauen und Umwelt e.V., 2016.
UNI EN ISO 9001:2015 September 2015, Quality (http://www.ibu-epd)
management systems - Requirements
OHSAS 18001
ISO 14001 OHSAS 18001:2007, Occupational Health and Safety
UNI EN ISO 14001:2015, Environmental management Management Certification.
systems - Requirements with guidance for use.
Ordinance on Biocide Products
Regulation (EU) No 528/2012 of the European
Further References Parliament and of the Council of 22 May 2012
concerning the making available on the market and
AgBB use of biocidal products.
Ausschuss zur gesundheitlichen Bewertung von
Bauprodukten, AgBB (eng. German Committee for PCR Part A
health-related evaluation of building products. PCR Part A: Calculation rules for the Life Cycle
Assessment and Requirements on the Background
BBSR Report according to EN 15 804+A2:2019, Version 1.0,
BBSR table "Service lives of components for life cycle Institut Bauen und Umwelt e.V., 2020.
assessment according to Bewertungssystem
Nachhaltiges Bauen (BNB)" Sustainable Building PCR Part B
Information Portal by the Federal Ministry of Transport, PCR Part B: requirements on the EPD for wood
Building and Urban Affairs (Bundesinstitut für Bau- cement - mineral-bonded wooden composites, version
,Stadt-und Raumforschung, BBSR). 1.7, Institut Bauen und Umwelt e.V., 2019.
(https://www.nachhaltigesbauen.de/baustoff-
undgebaeudedaten/ REACH Regulation
nutzungsdauern-von-bauteilen.html) Regulation (EU) No 1907/2006 of the European
Parliament and of the Council of 18 December 2006
Candidate list concerning the Registration, Evaluation, Authorisation
Candidate List of substances of very high concern for and Restriction of Chemicals (REACH), establishing a
Authorisation, published on ECHA website, latest European Chemicals Agency, amending Directive
version 19.01.2021. (https://echa.europa.eu/candidate- 1999/45/EC and repealing Council Regulation (EEC)
list-table) No 793/93 and Commission
Regulation (EC) No 1488/94 as well as Council
CPR Directive 76/769/EEC and Commission Directives
Construction Products Regulation, Regulation (EU) No 91/155/EEC, 93/67/EEC, 93/105/EC and 2000/21/EC.
305/2011 of the European Parliament and of the
Council of 9 March 2011 laying TA Luft
down harmonized conditions for the marketing of Technische Anleitung zur Reinhaltung der Luft, version
construction products and repealing Council Directive 16.12.2020.
89/106/ EEC Text with EEA relevance.
TRGS 900
Eurofins Product Testing A/S TRGS 900: Edition: January 2006
Eurofins Product Testing A/S, Smedeskovvej 38, 8464 BArBl. issue 1/2006 p. 41-55
Galten, Denmark. corrected GMBl 2020 S. 276 [No. 12-13] of 30.03.2020
amended and supplemented: GMBl 2020, 815-816
[No. 38] of 02.10.2020
GaBi ts software/ GaBi database https://www.baua.de/DE/Angebote/Rechtstexte-und-
GaBi Software System and Database for Life Cycle Technische-Regeln/Regelwerk/TRGS/TRGS-900.html
Engineering, 1992-2020, Sphera Solutions GmbH,
Leinfelden-Echterdingen, with acknowledgement of Waste Wood Ordinance
LBP University of Stuttgart, program version 9.5.2.49. Ordinance on requirements for the exploitation and
Database version 2020.1, SP40. disposal of waste wood of 15.08.2002.
GaBi documentation Umwelt Control Labor GmbH
GaBi dataset documentation for the software system Umwelt Control Labor GmbH, Postfach 2063, 44510
and databases, LBP, University of Stuttgart and Lünen, Deutschland.
Sphera Solutions GmbH, Leinfelden-Echterdingen,
2020.
(http://www.gabi-
software.com/international/support/gabi/gabi-database-
2020-lci-documentation/)
11 Environmental Product Declaration Etex Germany Exteriors GmbH – Duripanel A2
Publisher
Institut Bauen und Umwelt e.V. Tel +49 (0)30 3087748- 0
Panoramastr. 1 Fax +49 (0)30 3087748- 29
10178 Berlin Mail info@ibu-epd.com
Germany Web www.ibu-epd.com
Programme holder
Institut Bauen und Umwelt e.V. Tel +49 (0)30 - 3087748- 0
Panoramastr 1 Fax +49 (0)30 – 3087748 - 29
10178 Berlin Mail info@ibu-epd.com
Germany Web www.ibu-epd.com
Author of the Life Cycle
Assessment Tel +32 (0)15 71 82 83
Peggy Van De Velde Fax +32 (0)15 71 82 29
Bormstraat 24 Mail
2830 Tisselt peggy.vandevelde@etexgroup.c
Belgium om
Web www.etexgroup.com
Owner of the Declaration
Etex Building Performance Tel +32 2 778 12 11
International Fax +32 2 778 12 12
Marcel Demonque 500 r Mail info@etexgroup.com
84915 Avignon Cedex 9 Web http://www.etexgroup.com
France
