ENVIRONMENTAL PRODUCT DECLARATION
as per ISO 14025 and EN 15804
Owner of the Declaration ArcelorMittal Europe - Flat Products
Programme holder Institut Bauen und Umwelt e.V. (IBU)
Publisher Institut Bauen und Umwelt e.V. (IBU)
Declaration number EPD-ARC-20200027-CBD1-EN
ECO EPD Ref. No. ECO-00001269
Issue date 10.07.2020
Valid to 09.07.2025
Cold Rolled Steel Coils
ArcelorMittal Europe
www.ibu-epd.com | https://epd-online.com
Umwelt Produktdeklaration Name des Herstellers – Name des Produkts
General Information
ArcelorMittal Europe Cold Rolled Steel Coils
Programme holder Owner of the declaration
IBU – Institut Bauen und Umwelt e.V. ArcelorMittal Europe – Flat Products
Panoramastr. 1 24-26 Boulevard d’Avranches
10178 Berlin L-1160 Luxembourg
Germany Luxembourg
Declaration number Declared product / declared unit
EPD-ARC-20200027-CBD1-EN The declaration applies to 1 ton of cold rolled steel coil.
This declaration is based on the product Scope:
category rules: The Life Cycle Assessment is based on data collected
Structural steels, 07.2014 from the ArcelorMittal plants producing Cold Rolled
(PCR checked and approved by the SVR) Coils, representing 95 % of the annual production from
2015.
Issue date
10.07.2020 The owner of the declaration shall be liable for the
underlying information and evidence; the IBU shall not
be liable with respect to manufacturer information, life
Valid to
cycle assessment data and evidences.
09.07.2025
Verification
The standard EN 15804 serves as the core PCR
Independent verification of the declaration and data
according to ISO 14025:2010
Dipl. Ing. Hans Peters internally x externally
(chairman of Institut Bauen und Umwelt e.V.)
Dr. Alexander Röder Mr Carl-Otto Neven
(Managing Director Institut Bauen und Umwelt e.V.)) (Independent verifier appointed by SVR)
Product
Product description/Product definition conditions. For the application and use the respective
This Environmental Product Declaration refers to Cold national provisions apply.
Rolled Steel Coil, Slit Coil and Sheet including
Indaten® weathering steel, consisting of carbon Indaten® cold rolled steel offers improved resistance to
steel. The EPD results reflect the volume weighted atmospheric corrosion. Despite not being covered by a
average of these products. specific European standard, it is a thin gauge version
of the hot rolled steel defined in the EN 10025-5:2019 -
Cold Rolled Coils are produced in ArcelorMittal cold Hot rolled products of structural steels - Part 5:
rolling mill in which Hot Rolled Steel coils are Technical delivery conditions for structural steels with
continuously rolled between a series of stands of improved atmospheric corrosion resistance for
rotating cylinders, and then annealed, either on a Indaten®.
continuous annealing line or on batch annealing
facilities. Alloy composition and process parameters It is a fine-grain, high-strength structural steel that has
are set to guarantee the required grade. The coils are been optimised to give improved processing and in-
then delivered to manufacturers for shaping into end service performance.
products to be included in building works, generally to
precise dimensions, thereby avoiding losses on the
construction site. Application
Cold Rolled Coils can be used in various construction
Mean thickness value is at 1.5 mm but the declaration applications, such as:
covers the whole range from 0.4 mm up to 3 mm.  Construction: façade & cladding, roofing, sun
Width range is from 30 mm up to 1880 mm. screens & shades.
 Road equipment: safety barriers, protection
For the use and application, the product has a
equipment, sound insulation wall panels.
performance taking into consideration EN 10130:2006
- Cold rolled low carbon steel flat products for cold  Art sculpture & Other industrial applications:
forming - Technical delivery conditions or EN Containers & filters, etc.
10268+A1:2013 - Cold rolled steel flat products with
high yield strength for cold forming - Technical delivery
2 Environmental Product Declaration ArcelorMittal – Cold rolled steel coil
Cold-rolled coils and Indaten® coils are delivered in strength, durability and corrosion resistance. High
wide coils, slit coils or sheets. It can be processed by strength low alloyed (HSLA) carbon steel has a carbon
all conventional processing operations used for cold content lower than 0.2 %.
rolled: cutting, slitting, bending, drawing, clinching, The metallurgical composition of weathering steels
profiling, stamping, welding etc. includes less than 0.2 % carbon. Alloying elements
(mainly copper, chromium, nickel, phosphorus, silicon,
Indaten® Weathering steels offer improved resistance and manganese) typically comprise less than 5 % of
to corrosion thanks to the addition of copper during the steel.
manufacture.
Weathering steels are known as corrosion resistant
Additional alloying elements and specific thermal steels. Like standard carbon steels, weathering steels
treatments during annealing can be used to increase oxidise when exposed to the atmosphere. Due to their
the steel’s tensile strength or make forming processes specific chemistry, the corrosion rate of weathering
easier. steels is generally much lower than that of standard
carbon steel. To obtain the weathering features, those
Technical Data steel grades are including some alloys like Cu, Cr, Ni,
ArcelorMittal Europe Flat products is producing Cold P & Mo in quantities defined by the standards. The
Rolled Steel Coils in 6 mills. The EPD covers 95 % of possible chemical composition is defined in European
the total production in 2015. standard. Weathering steels can be classified into two
categories: those with limited phosphorous content
ArcelorMittal offers a full range of grades in compliance (typically less than 0.035 %); and those with a higher
with the EN 10130 to meet different applications. phosphorous content. Weathering steels with a
phosphorous content of between 0.06 and 0.15 % are
ArcelorMittal has also created Indaten® weathering identified by the letter P at the end of the product
steel grade to meet different applications. name.
High levels of phosphorous improves the corrosion
Constructional data resistance of weathering steels. Phosphorous is not
Name Value Unit used in heavy plate for structural uses as it can form
Density 7850 kg/m3 iron phosphide (FeP3) during welding. This can
Modulus of elasticity 210000 MPa hamper weldability and cause the weld zone to
Coefficient of thermal expansion 12 10-6K-1 become brittle. For this reason, phosphorous
Thermal conductivity 48 W/(mK) weathering steels are usually only available in
Melting point 1650 °C thicknesses lower than 12 mm.
Minimum yield strength 180 - 850 MPa
This product contains substances listed in the
candidate list (date: 26.2.2020) exceeding 0.1
Performance data of the product with respect to its percentage by mass: no
characteristics in accordance with the relevant
technical provision from standards EN 10130 or EN Reference service life
10268 (no CE-marking). A reference service life for cold rolled steel coil is not
declared. Cold rolled coil products are construction
Voluntary data: ArcelorMittal product catalogue – products with many different application purposes. The
document centre: lifetime therefore will be limited by the application as
https://industry.arcelormittal.com/productdocumentcent well as the service life of the work.
re
First structural steel projects using weathering steel
Base materials/Ancillary materials were completed 50 years ago in Europe and have
The chemical composition is in accordance with EN demonstrated a very low maintenance level and no
10130 or EN 10268. High strength low alloyed (HSLA) need for painting.
carbon steel has a carbon content lower than 0.2 %.
Yield strengths from 180 MPa up to 850 MPa are At the end of life, weathering steel products could be
available. recovered, recycled and sent to the steel mill.
Steel is mainly iron and carbon, with small amounts of
alloying elements. These elements modify the
chemical and physical properties of steel such as
LCA: Calculation rules
Declared Unit
This Environmental Product Declaration refers to Cold
Rolled Steel Coil, Slit Coil and Sheet including Declared unit
Indaten® weathering steel, consisting of carbon steel, Name Value Unit
as specified in Part B requirements on the EPD for Declared unit 1000 kg
Structural Steels. Conversion factor to 1 kg 0.001 -
Density 7850 kg/m3
3 Environmental Product Declaration ArcelorMittal – Cold rolled steel coil
System boundary Module C3 takes into account the sorting and
Type of the EPD: cradle-to-gate - with options. shredding of after-use steel that is recycled, as well as
Module A1-A3, Module C3 and module D were the non-recovered scrap due to sorting efficiency
considered. which is landfilled. A conservative value of 2 % landfill
is considered.
Modules A1-A3 of the Cold Rolled Steel Coil, Slit Coil
and Sheet including Indaten® weathering steel Module D refers to the End-of-Life of the steel coil,
production include the following: including reuse and recycling.
· The provision of resources, additives, and energy
· Transport of resources and additives to the Comparability
production site Basically, a comparison or an evaluation of EPD data
· Production processes on-site including energy, is only possible if all the data sets to be compared
production of additives, disposal of production were created according to EN 15804 and the building
residues, and consideration of related emissions context, respectively the product-specific
· Recycling of production/manufacturing scrap. Steel characteristics of performance, are taken into account.
scrap is assumed to reach the end-of-waste status
once it is shredded and sorted, thus becomes input to Gabi version 9.2 was used with Gabi Database SP35
the product system in the inventory. version 8.7 to calculate this EPD.
LCA: Scenarios and additional technical information
Current practice for the average Cold Rolled Steel Coil
consist of 98 % recycling and 2 % landfill according to
the /European Commission Technical Steel Research/.
End of life (C3)
Name Value Unit
Landfilling 2 %
Reuse, recovery and/or recycling potentials (D),
relevant scenario information
Name Value Unit
Recycling 98 %
4 Environmental Product Declaration ArcelorMittal – Cold rolled steel coil
LCA: Results
DESCRIPTION OF THE SYSTEM BOUNDARY (X = INCLUDED IN LCA; MND = MODULE NOT DECLARED;
MNR = MODULE NOT RELEVANT)
BENEFITS AND
CONSTRUCTI LOADS
PRODUCT STAGE ON PROCESS USE STAGE END OF LIFE STAGE BEYOND THE
STAGE SYSTEM
BOUNDARIES
5 Environmental Product Declaration ArcelorMittal – Cold rolled steel coil
lairetam
waR
ylppus tropsnarT
gnirutcafunaM
eht
morf
tropsnarT
etis
eht
ot
etag
ylbmessA esU
ecnanetniaM
riapeR
tnemecalpeR tnemhsibrufeR
ygrene
lanoitarepO esu
retaw
lanoitarepO esu
noitcurtsnoc-eD
noitilomed tropsnarT
gnissecorp
etsaW
lasopsiD -esueR -yrevoceR -gnilcyceR laitnetop
A1 A2 A3 A4 A5 B1 B2 B3 B4 B5 B6 B7 C1 C2 C3 C4 D
X X X MND MND MND MND MNR MNR MNR MND MND MND MND X MND X
RESULTS OF THE LCA - ENVIRONMENTAL IMPACT: 1 ton of cold rolled steel coil
Parameter Unit A1-A3 C3 D
Global warming potential [kg CO2-Eq.] 2.38E+3 2.00E+0 -1.65E+3
Depletion potential of the stratospheric ozone layer [kg CFC11-Eq.] 4.82E-9 6.89E-12 3.24E-10
Acidification potential of land and water [kg SO2-Eq.] 4.12E+0 6.78E-3 -3.98E+0
Eutrophication potential [kg (PO4)3--Eq.] 4.18E-1 7.99E-4 -3.41E-1
Formation potential of tropospheric ozone photochemical oxidants [kg ethene-Eq.] 7.04E-1 4.75E-4 -5.12E-1
Abiotic depletion potential for non-fossil resources [kg Sb-Eq.] 1.02E-4 9.53E-7 1.70E-4
Abiotic depletion potential for fossil resources [MJ] 2.06E+4 2.25E+1 -1.31E+4
RESULTS OF THE LCA - RESOURCE USE: 1 ton of cold rolled steel coil
Parameter Unit A1-A3 C3 D
Renewable primary energy as energy carrier [MJ] 6.16E+2 1.12E+1 1.20E+3
Renewable primary energy resources as material utilization [MJ] 0.00E+0 0.00E+0 0.00E+0
Total use of renewable primary energy resources [MJ] 6.16E+2 1.12E+1 1.20E+3
Non-renewable primary energy as energy carrier [MJ] 2.06E+4 3.43E+1 -1.23E+4
Non-renewable primary energy as material utilization [MJ] 0.00E+0 0.00E+0 0.00E+0
Total use of non-renewable primary energy resources [MJ] 2.06E+4 3.43E+1 -1.23E+4
Use of secondary material [kg] 1.13E+2 0.00E+0 0.00E+0
Use of renewable secondary fuels [MJ] 0.00E+0 0.00E+0 0.00E+0
Use of non-renewable secondary fuels [MJ] 0.00E+0 0.00E+0 0.00E+0
Use of net fresh water [m³] 4.59E+0 1.53E-2 5.79E-1
RESULTS OF THE LCA – OUTPUT FLOWS AND WASTE CATEGORIES:
1 ton of cold rolled steel coil
Parameter Unit A1-A3 C3 D
Hazardous waste disposed [kg] 1.37E-5 2.18E-7 -8.67E-6
Non-hazardous waste disposed [kg] 4.21E+0 2.01E+1 -2.63E+1
Radioactive waste disposed [kg] -2.71E-3 4.70E-3 2.94E-1
Components for re-use [kg] 0.00E+0 0.00E+0 0.00E+0
Materials for recycling [kg] 0.00E+0 9.80E+2 0.00E+0
Materials for energy recovery [kg] 0.00E+0 0.00E+0 0.00E+0
Exported electrical energy [MJ] 0.00E+0 0.00E+0 0.00E+0
Exported thermal energy [MJ] 0.00E+0 0.00E+0 0.00E+0
References
EN 10025 PCR Part B
EN 10025-5:2019 - Hot rolled products of structural PCR - Part B: Requirements of the EPD for Structural
steels - Part 5: Technical delivery conditions for steels,
structural steels with improved atmospheric corrosion Institut Bauen und Umwelt e.V., www.bauumwelt.com,
resistance 2017
EN 10130 Institut Bauen und Umwelt
EN 10130:2006 - Cold rolled low carbon steel flat Institut Bauen und Umwelt e.V., Berlin (pub.):
products for cold forming - Technical delivery Generation of Environmental Product Declarations
conditions (EPDs);
EN 10268 ISO 14025
EN 10268+A1:2013 - Cold rolled steel flat products DIN EN ISO 14025:2011-10 - Environmental labels
with high yield strength for cold forming - Technical and
delivery conditions declarations - Type III environmental declarations -
Principles and procedures
EN 15804 GaBi ts Documentation
EN 15804+A1:2013 - Sustainability of Documentation of the GaBi datasets for Life Cycle
construction works - Environmental Product Engineering. LBP, Universitity of Stuttgart and PE
Declarations - Core rules for the product category of International, 2017.
construction products http://documentation.gabi-software.com
European Commission Technical Steel Research REACH
Sansom, M.and Meijer, J.:Life-cycle Regulation (EC) No 1907/2006 of the European
assessment (LCA) for steel construction, European Parliament and of the Council on the Registration,
Commission technical steel research, 2001-12 Evaluation, Authorisation and Restriction
of Chemicals (REACH)
GaBi ts Software https://echa.europa.eu/regulations/reach/legislation
GaBi ts. Software and Databases
5 Environmental Product Declaration ArcelorMittal -
Organic coated steel coils Granite® and Estetic® for
Life Cycle Engineering. LBP, University of Stuttgart
und PE International, 2017.
6 Environmental Product Declaration ArcelorMittal – Cold rolled steel coil
Publisher
Institut Bauen und Umwelt e.V. Tel +49 (0)30 3087748- 0
Panoramastr. 1 Fax +49 (0)30 3087748- 29
10178 Berlin Mail info@ibu-epd.com
Germany Web www.ibu-epd.com
Programme holder
Institut Bauen und Umwelt e.V. Tel +49 (0)30 - 3087748- 0
Panoramastr 1 Fax +49 (0)30 – 3087748 - 29
10178 Berlin Mail info@ibu-epd.com
Germany Web www.ibu-epd.com
Author of the Life Cycle
Assessment Tel +352 4792-1
ArcelorMittal Europe – Flat Products Fax -
Boulevard d’Avranches 24-26 Mail
1160 Luxembourg flateurope.technical.assistance
Luxembourg @arcelormittal.com
Web flateurope.arcelormittal.com/
Owner of the Declaration
ArcelorMittal Europe – Flat Products Tel +352 4792-1
Boulevard d’Avranches 24-26 Fax -
1160 Luxembourg Mail
Luxembourg flateurope.technical.assistance
@arcelormittal.com
Web flateurope.arcelormittal.com/
