ENVIRONMENTAL PRODUCT DECLARATION
as per ISO 14025 and EN 15804+A2
Owner of the Declaration Gartner Extrusion GmbH
Publisher Institut Bauen und Umwelt e.V. (IBU)
Programme holder Institut Bauen und Umwelt e.V. (IBU)
Declaration number EPD-GAR-20230467-IBA1-EN
Issue date 14.12.2023
Valid to 13.12.2028
Aluminum profiles – composite, thermally-broken
Gartner Extrusion GmbH
www.ibu-epd.com | https://epd-online.com
1. General Information
Gartner Extrusion GmbH Aluminum profiles – composite, thermally-broken
Programme holder Owner of the declaration
IBU – Institut Bauen und Umwelt e.V. Gartner Extrusion GmbH
Hegelplatz 1 Peterswörther Straße 1a
10117 Berlin 89423 Gundelfingen
Germany Germany
Declaration number Declared product / declared unit
EPD-GAR-20230467-IBA1-EN 1 kg aluminum profile – composite, thermally-broken
This declaration is based on the product category rules: Scope:
Building metals, 01.08.2021 The EPD is based on annual production data for 2020 at the Gundelfingen
(PCR checked and approved by the SVR) site.
The owner of the declaration shall be liable for the underlying information
and evidence; the IBU shall not be liable with respect to manufacturer
Issue date information, life cycle assessment data and evidences.
14.12.2023
The EPD was created according to the specifications of EN 15804+A2. In
the following, the standard will be simplified as EN 15804.
Valid to
Verification
13.12.2028
The standard EN 15804 serves as the core PCR
Independent verification of the declaration and data according to ISO
14025:2011
internally X externally
Dipl.-Ing. Hans Peters
(Chairman of Institut Bauen und Umwelt e.V.)
Florian Pronold Dr. Eva Schmincke,
(Managing Director Institut Bauen und Umwelt e.V.) (Independent verifier)
1 Environmental Product Declaration - Gartner Extrusion GmbH - Aluminum profiles – composite, thermally-broken
2. Product
Name Value Unit
2.1 Product description/Product definition
Density 2700 kg/m3
The aluminium profiles produced are primarily used in the
construction industry, mechanical engineering, the automotive Melting point 660 °C
industry, electrical engineering and medical technology. The Elektrische Leitfähigkeit bei 20°C 28–34 m/Ω*mm2
starting materials are aluminium alloys made from the light Thermal conductivity 200–240 W/(mK)
metal aluminium (Al) and various alloying elements such as
Modulus of elasticity 70000 N/mm2
silicon, manganese, iron, magnesium etc. Depending on
customer requirements, the aluminium profiles can be supplied Thrust module 27000 N/mm2
surface-treated (anodised or powder-coated), mechanically- Specific thermal capacity 0,9–0,92 kJ/kgK
processed and/or thermally-broken. Hardness 40–100 HB
Yield strength Rp 0.2 60–300 N/mm2
Applicable standards:
Depending on whether aluminium profiles are load-bearing in
Tensile strength Rm 90–350 N/mm2
their end application or not (e.g. window frames, support Elongation at break 6–30 %
beams), they may or may not be subject to harmonisation
regulations. As aluminium profiles are intermediate products, it
Aluminium profiles and constructions according to CPR (hEN)
is often not possible to make a clear statement about their final
Performance values of the product according to the Declaration
applications. For this reason, both standards ('Profiles and
of Performance in terms of its essential characteristics in
constructions according to CPR' and 'Profiles not subject to EU
accordance with:
harmonisation regulations') are listed below. This covers the
range of possible final applications. • DIN EN 15088:2006-03, Aluminium and aluminium
alloys – Structural products for construction works –
Aluminium profiles and constructions according to CPR (hEN) Technical delivery conditions
(EU) Directive No. 305/2011 (CPR) applies for placing the
product on the market in the EU/EFTA (with the exception of Profiles which are not subject to any EU harmonisation
Switzerland). The product requires a Declaration of legalisation guidelines
Performance taking consideration of the following standards: Product performance values in terms of its characteristics
following the relevant technical determination (no CE marking).
• DIN EN 15088:2006-03, Aluminium and aluminium
alloys – Structural products for construction works – 2.4 Delivery status
Technical for inspection and delivery The aluminium profiles are supplied in accordance with EN
Use is governed by the respective national regulations. 755-1 or EN 12020-1. The chemical composition of the alloys is
based on EN 573-3.
Aluminium products which are not subject to any EU The packaging of the aluminium profiles is based on the
harmonisation guidelines customer's requirements. Reusable customer racks are just as
Application of the product is subject to the respective national conceivable as packaging made of cardboard, wood, plastic
guidelines at the place of use: film etc.
• DIN EN 755-1:2016-10, Aluminium and aluminium alloys
2.5 Base materials/Ancillary materials
– Extruded rods/bars, tubes and profiles – Part 1:
Technical conditions for inspection and delivery The chemical composition of the aluminium alloys used for
• DIN EN 12020-1:2022-05, Aluminium and aluminium aluminium profiles can be found in the EN 573-3 standard. The
alloys – Extruded precision profiles in alloys EN AW- aluminium content is more than 90%.
6060 and EN AW-6063 – Part 1: Technical conditions for
inspection and delivery The product / At least one sub-product contains substances
from the ECHA list of candidates of Substances of Very High
2.2 Application Concern (SVHC) (12.2023) exceeding 0.1% by mass: no
Due to their versatile properties, aluminium profiles can be used
in a wide variety of areas. In the construction sector, aluminium The product / At least one sub-product contains other CMR
profiles can be used for the production of facades, windows, substances in categories 1A or 1B which are not on the
doors, substructures etc.; in the automotive industry, for candidate list, exceeding 0.1% by mass in at least one sub-
example, as frames for sliding roofs or as roof rails; and in product: no
mechanical engineering, for example, as pneumatic profiles.
Biocide products were added to this construction product, or it
2.3 Technical Data has been treated with biocide products (this then concerns a
Physical properties of aluminium: treated product as defined by the (EU) Regulation on Biocide
Products No. 528/2012): no
Technical construction data
Explanation of aluminium (Al) as a material:
Aluminium is a silver-white light metal with a melting point of
660 °C.
Aluminium is covered by a natural, thin oxide layer and is
therefore protected from decomposition by air, water or certain
chemicals. This makes the material highly corrosion-resistant
and durable.
The properties of aluminium also make it possible to produce
profiles with complex shapes and contours. In addition,
2 Environmental Product Declaration - Gartner Extrusion GmbH - Aluminum profiles – composite, thermally-broken
aluminium is not only very corrosion-resistant, weldable and confirmed by the relevant employers' liability insurance
bendable, it is also a good heat conductor, a good electrical association, other authorities etc. on the one hand and by
conductor, and can be easily machined. Aluminium also has management systems such as ISO 14001, ISO 50001 etc. on
good casting properties. the other, and is continuously monitored by accredited
certification companies.
2.6 Manufacture
Heating in the billet furnace: The aluminium billet is heated to 2.8 Product processing/Installation
460 °C to 530 °C to enable the metal to reach its plastic state. Aluminium profiles are normally semi-finished products. This
means that processing to the end product is carried out by the
Extrusion moulding: In an extrusion plant, the heated respective customer and depends primarily on the intended
aluminium billet is pressed through a preheated pressing tool application of the individual customer.
with pressing forces of over 10 MN. This produces the various
contours of the aluminium profiles agreed with the customer. 2.9 Packaging
All aluminium profiles are packaged in accordance with agreed
Cooling the aluminium profiles: The profiles produced are customer requirements. The packaging variants used range
cooled directly after extrusion. There are various options for from reusable customer racks to untreated wooden crates and
this: air, water or spray mist. Cooling the aluminium profiles cardboard packaging.
affects the strength of the product, among other things. The separate packaging of the individual aluminium profiles,
e.g. using cardboard interlayers, polyethylene (PE) film, paper
Stretching the aluminium profiles: After extrusion and etc., is designed to provide optimum protection for the
cooling, the aluminium profiles are stretched. The profiles are aluminium profiles so that they do not incur any damage during
usually stretched beyond their elastic limit and thus transport.
straightened. The packaging materials used can be recycled by the customer.
2.10 Condition of use
Cutting the aluminium profiles to length: The aluminium
profiles are cut to length to meet customer requirements using The aluminium profiles are alloys with the specified alloy
a cold saw. components. The ingredients correspond to the basic materials
specified in EN 573-3 with their respective mass percentages.
Artificial ageing: Subsequent heat treatment of the aluminium There are no special features of the material composition for
profiles in artificial ageing furnaces (different temperature the period of use. For surface-treated aluminium profiles
ranges with coordinated duration) ensures that the required (anodised or powder-coated), the
mechanical properties are achieved. information/instructions/specifications of the respective quality
associations (e.g. GSB, Qualicoat, Qualanod) and the
Surface treatment: Surface treatment of the aluminium profiles specifications of the manufacturers of the powder coatings
(coating with powder paint or electrical oxidation, i.e. anodising) used must be observed (e.g. regarding corrosion resistance,
ensures that the appearance and corrosion requirements meet UV radiation etc.).
the customer's demands.
2.11 Environment and health during use
When the aluminium profiles are used as intended, no hazards
Thermal breaking: Building profiles in particular must fulfil high
can arise for water, air/atmosphere and soil.
thermal requirements. This is achieved by separating or
The requirements for use and maintenance are not based on
connecting the inner and outer profiles with one or more plastic
the semi-finished products manufactured, but on the specific
bars (with or without additional insulation between the inner and
design and application of the end product.
outer profiles).
2.12 Reference service life
Mechanical processing: Using state-of-the-art equipment, all
The reference service life (RSL) for aluminium profiles is not
mechanical processing operations agreed with the customer
declared, as these are semi-finished products with a wide range
are carried out on the aluminium profiles so that they can be
of possible applications. Use and further processing by the
used by the customer as planned.
manufacturer of the finished product are the decisive factors
here. A natural oxide layer that forms on the surface
Remelting production scrap: The production scrap incurred
permanently protects the aluminium from the effects of
during the manufacture of aluminium profiles is remelted
weathering and ageing.
directly on site in a remelting plant at approx. 750 °C. The
extrusion billets produced in this way are reused in the existing 2.13 Extraordinary effects
extrusion lines. This ensures a closed scrap cycle at the site, Fire
combined with all the energy benefits. Uncoated aluminium profiles comply with the requirements of
building material class A 'non-combustible', in accordance with
Packaging: Customised packaging of the aluminium profiles DIN 4102-4. The melting point for aluminium is 660 °C.
takes place at the end of the production process. The
• Smoke gas development: no smoke gas development
aluminium profiles are then ready for dispatch.
occurs with bare aluminium profiles
• Burning droplets: not applicable
All processes relating to the production of aluminium profiles
• Fire gas toxicity: not applicable
and the remelting of the resulting profile remnants are
monitored by certified quality management systems (e.g. ISO
9001, IATF 16949 etc.) with regard to qualitative product Water
requirements in accordance with standards. The effects of water on the aluminium profiles do not lead to
any changes in the product or any other negative
2.7 Environment and health during manufacturing environmental impact.
During the entire manufacturing process described above, all
legal obligations regarding occupational safety, health and Mechanical destruction
safety, energy and the environment are complied with. This is Mechanical destruction is not of relevance for aluminium
3 Environmental Product Declaration - Gartner Extrusion GmbH - Aluminum profiles – composite, thermally-broken
profiles. product.
Due to its high value, aluminium scrap is recycled as a raw
2.14 Re-use phase material and fed into an established cycle for reuse.
Bare aluminium profiles in particular are 100% recyclable The energy consumption during the recycling of aluminium
without any loss of quality. Coated scrap and scrap from profiles corresponds to only approx. 5% of the original energy
demolition, conversion or refurbishment can be easily consumption required for the production of primary aluminium.
separated and fed into the recycling process (via the recycling If aluminium profiles are nevertheless sent to landfill, there is no
industry). environmental impact.
2.15 Disposal 2.16 Further information
According to the European Waste Catalogue (EWC), waste Please refer to www.gutmann.de.
classification (waste code) is based on the respective end
3. LCA: Calculation rules
powder-coated, thermally-broken and mechanically processed.
3.1 Declared Unit
The declared unit refers to aluminium profiles produced by
Gartner Extrusion GmbH in Gundelfingen, Germany.
This EPD specifies the declared unit as 1 kg of aluminium
profiles in the 'composite, thermally-broken' finishing stage.
Declared unit and mass reference
Name Value Unit
Declared unit 1 kg
The products analysed are almost identical in terms of their
basic composition and processing. The declared results are
therefore highly representative.
3.2 System boundary
The analysis is designed as a 'cradle-to-gate with options'
approach. In particular, the production from the raw materials to
the finished product ('cradle-to-gate') is taken into account. In
addition, the expenses for recycling are included for disposal at
the end of the life cycle. Any credits incurred for the secondary
product from material recycling are shown separately. The
transport of the profiles ex works, any further processing as well
as installation, dismantling and return transport are not included
in the analysis.
The following aluminium profile production processes are taken
into account in modules A1–A3:
• Provision of raw, ancillary and operating materials and
energy
• Transport of materials to the plant and removal of Due to the low environmental impact of the packaging, its
residual materials disposal is not taken into account in Module A5.
• Disposal of residual materials At the end of the life cycle of the aluminium profiles, the
• Directly occurring emissions following processes are taken into account for the disposal
Particular attention is paid to: stage:
• the external production of purchased aluminium billets, • C3: Shredding of the aluminium scrap. The end-of-
profiles and ingots waste property is reached after shredding.
• the manufacturing processes of the aluminium profiles • D: The shredded scrap is remelted into secondary
in the plant – depending on the aluminium profile aluminium. The environmental credit for the net scrap
product class, including surface finishing and quantity is offset against the expenses saved by
mechanical post-processing substituting primary aluminium.
• the consumption of other operating materials (tools,
3.3 Estimates and assumptions
cleaning agents, industrial gases)
• the consumption of packaging materials (foils, In the absence of a representative underlying data set,
cardboard, steel straps and wooden pallets) estimates and assumptions are used for modelling purposes.
• the assumption of closed-loop recycling in the melting These are documented accordingly.
furnace for the aluminium production waste generated
3.4 Cut-off criteria
at the site (direct reuse as raw material possible, as the
The LCA model contains all relevant input and output data for
scrap does not suffer any loss of quality)
which information is available. Data gaps were filled with
conservative assumptions (average data or generic data) where
The following figure schematically shows the sub-processes
data was available.
considered for A1 to A3: remelting, extrusion, anodising and
Only material flows with a contribution of less than 1% of the
surface coating. This analysis is supplemented with data on the
mass input in relation to the respective sub-process step were
remaining overall operation. Five types of aluminium profiles
cut off, but only on the condition that the anticipated effect is
are produced at the Gundelfingen site: mill-finished, anodised,
likely to be insignificant.
4 Environmental Product Declaration - Gartner Extrusion GmbH - Aluminum profiles – composite, thermally-broken
No processes, materials or emissions were neglected that
make a significant contribution to the environmental impact of 3.7 Period under review
the products analysed. The total sum of the neglected input and Data for the 2020 production year was used for data collection.
output flows in relation to the total quantity of aluminium used
3.8 Geographic Representativeness
(17,000 tonnes) is no more than 0.5% by mass.
Land or region, in which the declared product system is
3.5 Background data manufactured, used or handled at the end of the product´s
The LCA for Experts (GaBi) software system is used to model lifespan: Germany
the life cycle of the products under consideration. The data
required for both upstream and downstream processes is taken
3.9 Allocation
from the Sphera LCA databases, version 2023.1 (Sphera
An allocation of co-products was avoided. Quantities of
2023).
aluminium dross and aluminium hydroxide are included in the
3.6 Data quality analysis by extending the system boundary in the
For the life cycle inventory of the primary data, the annual corresponding remelting and anodising sub-process steps. The
quantities used and produced and the consumption of energy environmental impacts of the remelting and extrusion sub-
and the required raw materials and supplies at the processes are allocated to the respective downstream process
Gundelfingen site were recorded. Further questions were steps via the mass fractions of the material quantities. The
clarified in the subsequent iterative process. The material and allocation of resources (material and energy use) for the
energy flows for the production site are realistically mapped remaining overall operation is carried out for the end products
thanks to in-depth discussions between the life cycle assessor based on their mass share of the total product quantity.
bifa Umweltinstitut GmbH and Gartner Extrusion GmbH. Multi-input processes are not relevant for this analysis.
In order to determine the net flows of aluminium into material
Due to the detailed data collection (metre and ERP system, recycling, the quantity of external aluminium scrap used in A1 to
balance sheet data) and the review process, it can be assumed A3 is deducted from the total quantity of end-of-life products in
that the primary data collected is of very high quality. accordance with the requirements of PCR, Part B.
3.10 Comparability
When selecting the background data, care was taken to
Basically, a comparison or an evaluation of EPD data is only
ensure technical, geographical and time-related
possible if all the data sets to be compared were created
representativeness. Missing data was approximated using
according to EN 15804 and the building context, respectively
generic data sets or representative average values. The
the product-specific characteristics of performance, are taken
underlying data sets used are not older than ten years.
into account. See point 3.5 for details of the calculation.
4. LCA: Scenarios and additional technical information
As the aluminium profiles are semi-finished products, the
Characteristic product properties of biogenic carbon reference service life is not declared (see section 2.12).
The product aluminium profile – composite, thermally-broken
End of Life (C1-C4)
does not contain any biogenic carbon.
The proportion of biogenic carbon in the associated packaging Name Value Unit
is 0.016 kg. Collected separately waste type 1 kg
Note: 1 kg of biogenic carbon is equivalent to 44/12 kg of CO 2. Recycling 0.96 kg
Landfilling 0.04 kg
For extruded aluminium profiles, it is assumed that 96% by
The following technical information forms the basis for the
mass will be recycled at their end of life.
declared modules or can be used for developing specific
scenarios in the context of a building evaluation if modules are
not declared (MND). Reuse, recovery and recycling potential (D), relevant
scenario details
Construction installation process (A5)
Name Value Unit
The use of packaging material is balanced in module A3 for the
declared product, but disposal of the packaging material is not Recycling efficiency Al remelting 0,98 kg
declared in module A5. The following table shows the balanced
quantities of packaging materials as technical information for
The declared products are semi-finished products whose end of
module A5.
life depends heavily on their use as end products. This is
Name Value Unit therefore a consistent assumption in the context of building
Wood packaging 0,022 kg certification. Primary aluminium is substituted when the product
is recycled.
PE foil packaging 0,002 kg
Cardboard packaging 0,017 kg
5 Environmental Product Declaration - Gartner Extrusion GmbH - Aluminum profiles – composite, thermally-broken
5. LCA: Results
For a declared unit of 1 kg of aluminium profile – composite, thermally-broken, the indicators for the Life Cycle Inventory and
impact assessment in accordance with EN 15804 are listed below. The additional impact categories according to EN 15804+A2
(optional) are not shown.
DESCRIPTION OF THE SYSTEM BOUNDARY (X = INCLUDED IN LCA; MND = MODULE OR INDICATOR NOT DECLARED; MNR
= MODULE NOT RELEVANT)
Benefits and
Construction loads beyond
Product stage Use stage End of life stage
process stage the system
boundaries
la ire ta m w a Ry lp p u s tro p s n a rT g n iru tc a fu n a M e h t m o rf tro p s n a rTe tis e h t o t e ta g y lb m e s s A e s U e c n a n e tn ia M ria p e R tn e m e c a lp e R tn e m h s ib ru fe R y g re n e la n o ita re p Oe s u re ta w la n o ita re p Oe s u n o itc u rts n o c -e Dn o itilo m e d tro p s n a rT g n is s e c o rp e ts a W la s o p s iD -e s u e R-y re v o c e R-g n ilc y c e Rla itn e to p
A1 A2 A3 A4 A5 B1 B2 B3 B4 B5 B6 B7 C1 C2 C3 C4 D
X X X MND MND MND MND MNR MNR MNR MND MND MND MND X MND X
RESULTS OF THE LCA - ENVIRONMENTAL IMPACT according to EN 15804+A2: 1 kg Aluminum profiles – composite,
thermally-broken
Parameter Unit A1-A3 C3 D
Global Warming Potential total (GWP-total) kg CO 2 eq 5.18E+00 8.49E-03 -3.06E+00
Global Warming Potential fossil fuels (GWP-fossil) kg CO 2 eq 5.19E+00 8.39E-03 -3.05E+00
Global Warming Potential biogenic (GWP-biogenic) kg CO 2 eq -1.34E-02 9.12E-05 -9.81E-03
Global Warming Potential luluc (GWP-luluc) kg CO 2 eq 1.27E-03 9.05E-07 -6.01E-04
Depletion potential of the stratospheric ozone layer (ODP) kg CFC11 eq 3.01E-11 1.53E-13 -2.52E-11
Acidification potential of land and water (AP) mol H+ eq 1.56E-02 1.77E-05 -1.2E-02
Eutrophication potential aquatic freshwater (EP-freshwater) kg P eq 3.68E-06 3.11E-08 -1.54E-06
Eutrophication potential aquatic marine (EP-marine) kg N eq 2.76E-03 4.24E-06 -1.7E-03
Eutrophication potential terrestrial (EP-terrestrial) mol N eq 3E-02 4.43E-05 -1.84E-02
kg NMVOC
Formation potential of tropospheric ozone photochemical oxidants (POCP) 8.31E-03 1.13E-05 -5.25E-03
eq
Abiotic depletion potential for non fossil resources (ADPE) kg Sb eq 9.2E-07 1.29E-09 -8.49E-07
Abiotic depletion potential for fossil resources (ADPF) MJ 7.45E+01 1.74E-01 -4.39E+01
m3 world eq
Water use (WDP) 2.28E-01 1.83E-03 -1.33E-01
deprived
RESULTS OF THE LCA - INDICATORS TO DESCRIBE RESOURCE USE according to EN 15804+A2: 1 kg Aluminum profiles –
composite, thermally-broken
Parameter Unit A1-A3 C3 D
Renewable primary energy as energy carrier (PERE) MJ 2.6E+01 1.04E-01 -2.13E+01
Renewable primary energy resources as material utilization (PERM) MJ 1.73E-01 0 0
Total use of renewable primary energy resources (PERT) MJ 2.62E+01 1.04E-01 -2.13E+01
Non renewable primary energy as energy carrier (PENRE) MJ 7.37E+01 1.74E-01 -4.4E+01
Non renewable primary energy as material utilization (PENRM) MJ 8.6E-01 0 0
Total use of non renewable primary energy resources (PENRT) MJ 7.45E+01 1.74E-01 -4.4E+01
Use of secondary material (SM) kg 4.24E-01 0 0
Use of renewable secondary fuels (RSF) MJ 0 0 0
Use of non renewable secondary fuels (NRSF) MJ 0 0 0
Use of net fresh water (FW) m3 4.42E-02 8.39E-05 -3.7E-02
RESULTS OF THE LCA – WASTE CATEGORIES AND OUTPUT FLOWS according to EN 15804+A2:
1 kg Aluminum profiles – composite, thermally-broken
Parameter Unit A1-A3 C3 D
Hazardous waste disposed (HWD) kg 3.67E-08 2.18E-11 -2.8E-08
Non hazardous waste disposed (NHWD) kg 1.03E+00 1.28E-04 -9.14E-01
Radioactive waste disposed (RWD) kg 5.62E-03 2.77E-05 -5.02E-03
Components for re-use (CRU) kg 0 0 0
Materials for recycling (MFR) kg 0 9.6E-01 0
Materials for energy recovery (MER) kg 0 0 0
Exported electrical energy (EEE) MJ 0 0 0
Exported thermal energy (EET) MJ 0 0 0
RESULTS OF THE LCA – additional impact categories according to EN 15804+A2-optional:
1 kg Aluminum profiles – composite, thermally-broken
Parameter Unit A1-A3 C3 D
Disease
Incidence of disease due to PM emissions (PM) ND ND ND
incidence
6 Environmental Product Declaration - Gartner Extrusion GmbH - Aluminum profiles – composite, thermally-broken
Human exposure efficiency relative to U235 (IR) kBq U235 eq ND ND ND
Comparative toxic unit for ecosystems (ETP-fw) CTUe ND ND ND
Comparative toxic unit for humans (carcinogenic) (HTP-c) CTUh ND ND ND
Comparative toxic unit for humans (noncarcinogenic) (HTP-nc) CTUh ND ND ND
Soil quality index (SQP) SQP ND ND ND
Disclaimer – for the indicators 'abiotic depletion potential for non-fossil resources', 'abiotic depletion potential for fossil resources',
'water (user) deprivation potential, deprivation-weighted water consumption', 'potential comparative toxic unit for ecosystems', 'potential
comparative toxic unit for humans – cancerogenic', 'Potential comparative toxic unit for humans - not cancerogenic', 'potential soil
quality index'. The results of this environmental impact indicator shall be used with care as the uncertainties on these results are high
as there is limited experience with the indicator.
6. LCA: Interpretation
The following interpretation summarises the results of the Life adjusted accordingly.
Cycle Assessment for a defined quantity of 1 kg aluminium
profile – composite, thermally-broken. The results of the sectoral analyses carried out show that the
effects from production of the additional primary aluminium
The production phase (modules A1–A3) of the aluminium required through the purchase of aluminium ingots, billets and
profiles dominates the results in relation to the individual profiles contribute significantly to how environmentally friendly
phases. The environmental impacts are mainly influenced by the aluminium profiles described are. The statement applies
the upstream processes for the aluminium ingots, billets and accordingly to the recycling potential of remelting aluminium.
profiles used. In the biogenic climate change category, this
influence is more than compensated for by the storage of
carbon in the wood used for the packaging and the overall
result shows an environmental relief (negative). If the wooden
packaging is thermally utilised after use in module A5, the
resulting CO emissions must be included accordingly.
2
As other EPDs for aluminium products also show, the
environmental impact in module C is negligible compared to
A1–A3. The waste treatment by shredding shown at the end of
the product life cycle (module C3) only contributes very little to
the overall environmental impact of the products.
Due to the very good recyclability of aluminium, the material
can replace primary aluminium after recycling. Module D shows
the potential for recycling aluminium at the end of the product
life cycle. As a high proportion of secondary aluminium is
already used in the primary products of aluminium profiles, the
net flow into module D is reduced by these quantities. The
potential for substituting primary aluminium (credits) was
7. Requisite evidence
As semi-finished products offer a wide range of possible responsibility of the manufacturer of the final product.
applications, the design for use in further processing is the
8. References
Standards: DIN EN 12020-1:2022-05, Aluminium and aluminium alloys –
Extruded precision profiles in alloys EN AW-6060 and EN AW-
DIN 4102 6063 – Part 1: Technical delivery conditions
DIN 4102-4:2016-05, Fire behaviour of building materials and
building components – Part 4: Synopsis and application of EN 15088
classified building materials, components and special DIN EN 15088:2006-03, Aluminium and aluminium alloys –
components Structural products for construction works – Technical delivery
conditions
EN 573-3
DIN EN 573-3:2019-10, Aluminium and aluminium alloys – EN 15804
Chemical composition and form of wrought products – Part 3: EN 15804:2012+A2:2019+AC:2021, Sustainability of
Chemical composition and product forms construction works – Environmental product declarations –
Core rules for the product category of construction products
EN 755-1
DIN EN 755-1:2016-10, Aluminium and aluminium alloys – IATF 16949
Extruded rods/bars, tubes and profiles – Part 1: Technical Requirements on quality management systems for serial and
delivery conditions spare parts production in the automotive industry
EN 12020-1 ISO 9001
7 Environmental Product Declaration - Gartner Extrusion GmbH - Aluminum profiles – composite, thermally-broken
EN ISO 9001:2015, Quality management systems – EA 2018
Requirements European Aluminium: European Aluminium Environmental
Profile Report. Brussels, 2018, https://www.european-
ISO 14001 aluminium.eu/resource-hub/environmental-profile-report-2018/
EN ISO 14001:2015, Environmental management systems –
Requirements with guidance for use IBU 2021
General instructions for the EPD range of Institut Bauen und
ISO 14025 Umwelt e.V., Version 2.0, Berlin: Institut Bauen und Umwelt
EN ISO 14025:2011, Environmental designations and e.V., 2021, http://www.ibu-epd.com
declarations – Type III environmental declarations – Basic
principles and processes PCR Teil A
Product category rules for building-related products and
ISO 14040 services, Part A: Calculation rules for the Life Cycle
EN ISO 14040:2006+A1:2020, Environmental management – Assessment and requirements on the project report in
Life cycle assessment – Principles and framework accordance with EN
15804+A2:2019, version 1.3; Berlin: Institut Bauen und Umwelt
ISO 14044 e.V., 2022
EN ISO 14044:2006+A1:2018+A2:2020, Environmental
management – Life cycle assessment – Requirements and PCR Teil B
guidelines Product category guidelines for building-related products and
services, Part B: Requirements on the EPD for products made
ISO 50001 from aluminium and aluminium alloys, version 3; Berlin: Institut
EN ISO 50001:2018, Environmental management systems – Bauen und Umwelt e.V. (pub.), 2023
Requirements with guidance for use
Sphera 2023
Sphera Solutions, Inc.: LCA for Experts 10.7, Content 2023.1,
Other literature: LCA database server; Chicago, 2023,
https://scn.spherasolutions.com (registration required)
8 Environmental Product Declaration - Gartner Extrusion GmbH - Aluminum profiles – composite, thermally-broken
Publisher
Institut Bauen und Umwelt e.V. +49 (0)30 3087748- 0
Hegelplatz 1 info@ibu-epd.com
10117 Berlin www.ibu-epd.com
Germany
Programme holder
Institut Bauen und Umwelt e.V. +49 (0)30 3087748- 0
Hegelplatz 1 info@ibu-epd.com
10117 Berlin www.ibu-epd.com
Germany
Author of the Life Cycle Assessment
bifa Umweltinstitut GmbH +49 (0)821 7000-0
Am Mittleren Moos 46 solutions@bifa.de
86167 Augsburg www.bifa.de
Germany
Owner of the Declaration
Gartner Extrusion GmbH +49 (0)9073 8000-0
Peterswörther Straße 1a gartner@gutmann-group.com
89423 Gundelfingen www.gutmann.de
Germany
9 Environmental Product Declaration - Gartner Extrusion GmbH - Aluminum profiles – composite, thermally-broken
