ENVIRONMENTAL PRODUCT DECLARATION
as per ISO 14025 and EN 15804+A2
Owner of the Declaration Etex Building Performance International
Publisher Institut Bauen und Umwelt e.V. (IBU)
Programme holder Institut Bauen und Umwelt e.V. (IBU)
Declaration number EPD-ETE-20230096-IBA1-EN
Issue date 14.06.2023
Valid to 13.06.2028
MICROTHERM® Flexible panels range: (Semi-)Overstitched
Panels, (Semi-)Quilted Panels, Slatted Panels, Aeroguard (>160
kg/m3) and Slimflex
ETEX
www.ibu-epd.com | https://epd-online.com
1. General Information
ETEX MICROTHERM® Flexible panels range:
(Semi-)Overstitched Panels, (Semi-)Quilted
Panels, Slatted Panels, Aeroguard (>160 kg/m3)
and Slimflex
Programme holder Owner of the declaration
IBU – Institut Bauen und Umwelt e.V. Etex Building Performance International
Hegelplatz 1 Rue Marcel Demonque 500
10117 Berlin 84915 Avignon Cedex 9
Germany France
Declaration number Declared product / declared unit
EPD-ETE-20230096-IBA1-EN 1 m2 of MICROTHERM® Flexible panels range, including
(Semi-)Overstitched Panels, (Semi-)Quilted Panels, Slatted Panels,
Aeroguard (>160 kg/m3) and Slimflex
This declaration is based on the product category rules: Scope:
Mineral insulating materials, 01.08.2021 This product is representative for the MICROTHERM® Flexible panels
(PCR checked and approved by the SVR) range, including (Semi-)Overstitched Panels, (Semi-)Quilted Panels,
Slatted Panels, Aeroguard (>160 kg/m3) and Slimflex, produced by
MICROTHERM® (part of ETEX group) in Sint-Niklaas, Belgium.
Issue date The reference product used for this EPD is the MICROTHERM®
Overstitched panel 1000R and 1000R HY with a density of 220 kg/m3 and
14.06.2023
a thickness of 10 mm. A variability study has been performed in the LCA
background report to prove the representativeness.
The owner of the declaration shall be liable for the underlying information
Valid to
and evidence; the IBU shall not be liable with respect to manufacturer
13.06.2028 information, life cycle assessment data and evidences.
The EPD was created according to the specifications of EN 15804+A2. In
the following, the standard will be simplified as EN 15804.
Verification
The standard EN 15804 serves as the core PCR
Independent verification of the declaration and data according to ISO
14025:2011
internally X externally
Dipl.-Ing. Hans Peters
(Chairman of Institut Bauen und Umwelt e.V.)
Dipl.-Ing. Hans Peters Vito D'Incognito,
(Managing Director Institut Bauen und Umwelt e.V.) (Independent verifier)
Environmental-Product Declaration - ETEX - MICROTHERM® Flexible panels range: (Semi-)Overstitched Panels, (Semi-)Quilted Panels, Slatted Panels, Aeroguard
1 (>160 kg/m3) and Slimflex
2. Product
• automotive: exhaust, muffler
2.1 Product description/Product definition
This EPD covers the MICROTHERM® flexible panels: MARINE
(Semi-)Overstitched Panels, (Semi-)Quilted Panels, Slatted • exhaust systems
Panels, Aeroguard (> 160 kg/m3) and Slimflex range. These • engines
products are custom-made flexible microporous insulation
panels. The panels are produced in a glass cloth outer 2.3 Technical Data
envelope, making them clean and easy to handle. Stitching can Technical data
be one-directional (2D flexure), or two-directional (3D flexure).
Name Value Unit
The formulation is an opacified blend of filament-reinforced
Thermal conductivity at 200 °C 0.025 - 0.035 W/mK
pyrogenic silica (alumina for 1200 grade). Some products use
hydrophobic silica in the core to repel water. It is ideal for Gross density 160 - 350 kg/m3
applications where contact with liquid water or condensation Compressive strength 0.12 - 0.22 N/mm2
(dew point) is possible.
No EN or ETA norm for flexible panels as these products are
No EN or ETA norm for flexible panels as these products are not used in building & construction.
not used in building & construction.
2.4 Delivery status
2.2 Application
Microporous insulation offers (an) extremely low thermal
conductivity, close to the lowest theoretically possible at high
temperatures. Microporous materials are the preferred choice
when a large temperature reduction is required within a limited
space, or when strict heat loss or surface temperature
requirements are specified. Some specific examples of the
application areas are provided in the table below.
OIL AND GAS
• petrochemical industry
• piping insulation
2.5 Base materials/Ancillary materials
• back-up insulation in refractory lined pipes
• hot pipe support insulation Composition:
• filler material for mattresses • (Hydrophobic) Fumed silica
• cassettes • Rutile
• expansion joints • Glass fibre
• PFP (Passive Fire Protection) • Fumed alumina
• piping insulation (ideal for large diameters) • Others
• back-up insulation in refractory lined pipes vessels and
reactors This product/article/at least one partial article contains
substances listed in the candidate list (date: 16.12.2022)
ENERGY exceeding 0.1 percentage by mass: no
• turbine insulation This product/article/at least one partial article contains other
• pipe insulation carcinogenic, mutagenic, reprotoxic (CMR) substances in
• small radius pipe insulation categories 1A or 1B which are not on the candidate list,
• R&D centres – advanced research exceeding 0.1 percentage by mass: no
• fuel cells
• piping insulation in power stations Biocide products were added to this construction product or it
has been treated with biocide products (this then concerns a
HEAVY INDUSTRY treated product as defined by the (EU) Ordinance on Biocide
• rotary kiln insulation Products No. 528/2012): no
• exhaust system
• hot air valves 2.6 Manufacture
• exhaust systems The production of microporous flexible panels goes through
different steps. First of all the E-glass cloth bags are produced.
TRANSPORTATION They are cut to size from a roll, folded in 2 and stitched at 2
• thermalbatteries sides so one side is still open. In the meantime the raw
• exhaust systems materials are mixed together to get the appropriate mix, this is
• PFP of train floors done on the mixing platform. From there the mix is sent to the
• heat shields filling station where the right amount of mix is filled into the
• 3D geometries glass cloth bag and the bag is closed at the 4 sides. This bag
• aerospace with the mix inside is then pressed in the pressing hall to the
• Engine nacelles & thrust reversers required thickness. After this step the panels go to the multi-
needle where they are stitched in 1 or 2 directions to get a
Environmental-Product Declaration - ETEX - MICROTHERM® Flexible panels range: (Semi-)Overstitched Panels, (Semi-)Quilted Panels, Slatted Panels, Aeroguard
2 (>160 kg/m3) and Slimflex
flexible panel. These panels can be manipulated or machined
Fire protection
or are the final product to be packed.
Name Value
2.7 Environment and health during manufacturing Building material class A1
Environmental, occupational health, safety and quality Burning droplets Not available /
management at the Sint-Niklaas plant are in accordance with
Smoke gas development Not available /
the following standards:
• ISO 14001;2015
Water
• ISO 9001;2015
Tests on the product performance including possible impacts on
• ISO 45001:2018
the environment following the unforeseeable influence of water,
2.8 Product processing/Installation e.g. flooding showed that no risks are expected to occur in
terms of environment and human health.
Not considered in the scope of the EPD, as a wide range of
different applications and installation scenarios can be applied.
Mechanical destruction
2.9 Packaging In the case of mechanical destruction, no risks are expected to
A wooden pallet, carton and plastic packaging are used to pack occur in terms of environment and human health.
the product for transport to the installation/customer.
2.14 Re-use phase
2.10 Condition of use No reuse/recycling has been considered.
No maintenance is needed.
2.15 Disposal
2.11 Environment and health during use Waste from these materials may be generally disposed off at a
Under normal conditions of use, MICROTHERM panels do not landfill, which has been licensed for this purpose. Please refer
cause any adverse health effects or release of volatile organic to the European list (Decision N° 2000/532/CE as modified) to
compounds (VOCs) into indoor air. No environmental impact on identify your appropriate waste number, and ensure national
water, air or soil is expected due to the extremely low metal and/or regional regulations are complied with.
release from the low maintenance requirements. Unless wetted, such a waste is normally dusty and so should
be properly sealed in containers for disposal. At some
2.12 Reference service life authorised disposal sites, dusty waste may be treated
The reference service life is not declared, as the EPD does not differently in order to ensure they are dealt with promptly to
cover the use stage. The RSL depends on the application. avoid them being windblown. Check for any national and/or
Under normal conditions of use, the product is supposed to regional regulations, which may apply.
remain its characteristics as long as the application lasts.
2.16 Further information
2.13 Extraordinary effects Additional information on MICROTHERM® Flexible panels can
Fire be found at:
All microporous products are A1 non-combustible according https://www.promat.com/en/industry/technologies/microporous-
EN13501, materials/high-temperature-insulation/
3. LCA: Calculation rules
compared to the core, one can still use the formula below.
3.1 Declared Unit
The declared unit is defined as: 1 m2 (thickness 10 mm) of a E = W*E /W
ref ref
MICROTHERM® Flexible panel with a thermal conductivity
between 0.025-0.035 W/mK at 200 °C. E = environmental impact of a product with density d and
Declared unit thickness t
Name Value Unit
W = d*t = weight of 1 m2 product with density d and thickness t
Declared unit 2.2 kg
Gross density 220 kg/m3
E = environmental impact of the reference product with
ref
Grammage 2.2 kg/m2 density 220 kg/m3 and thickness 10 mm
Layer thickness 0.01 m
W = weight of 1 m2 reference product with density 220 kg/m3
The reference product used for this EPD is the ref
MICROTHERM® Overstitched panel 1000R and 1000R HY and thickness 10 mm
with a density of 220 kg/m3 and a thickness of 10 mm.
3.2 System boundary
cradle to gate - with options, valid for the European market.
A variability study has been performed in the LCA background
report to describe the variance with the other products included
3.3 Estimates and assumptions
in the EPD, i.e. Quilted Panels, Slatted Panels, Aeroguard
No data record for (hydrophobic) fumed silica and fumed
(>160 kg/m3) and Slimflex.
alumina is available in Ecoinvent. Therefore, a customized
model has been used, based on the stoichiometry of the
The environmental impact of a product can be considered to be
chemical reaction and energy consumption provided by ETEX's
proportional to the weight of the product, so products with
supplier. During the production of fumed silica and fumed
another density and/or thickness can be calculated by the
alumina, Hydrogen chloride (HCl) is produced as a co-product.
below formula. Note that the glass fibre is not proportional to
Impacts have been allocated on an economic basis to both end
the thickness, but to the surface area instead. However, as the
products (fumed silica and HCl).
glass fibre as little contribution to the environmental impact
Environmental-Product Declaration - ETEX - MICROTHERM® Flexible panels range: (Semi-)Overstitched Panels, (Semi-)Quilted Panels, Slatted Panels, Aeroguard
3 (>160 kg/m3) and Slimflex
3.4 Cut-off criteria 3.7 Period under review
The following processes are considered below cut-off: The data collected by MICROTHERM® are based on data from
the year 2021.
• Transport of packaging of raw materials
• Infrastructure and land use of the factory
3.8 Geographic Representativeness
• Ancillary materials used during the manufacturing
Land or region, in which the declared product system is
• Environmental impacts caused by the personnel of the
manufactured, used or handled at the end of the product´s
production plants are not included in the LCA, e.g.
lifespan: Europe
waste from the cafeteria and sanitary installations,
accidental pollution caused by human mistakes, or
environmental effects caused by commuter traffic. 3.9 Allocation
Heating or cooling of the plants in order to ensure a
No co-products are produced.
comfortable indoor climate for the personnel for
No secondary raw materials are used.
example is also neglected.
The following allocations have been considered for the
3.5 Background data
production data:
Ecoinvent 3.8 and Industry 2.0
• For the energy consumption specific data per production
3.6 Data quality step was available. The production steps have been
Company-specific data concern the data about the production divided into steps that are common to all the products
of MICROTHERM® Flexible panels range. All required data produced in the plant in Sint-Niklaas and steps that are
about the production process have been delivered to Enperas specific to certain products. The energy consumption of
by MICROTHERM®. Enperas uses publicly available generic the common production steps has been allocated to the
data for all background processes (Ecoinvent 3.8 and Industry individual product using the annual production volume of
2.0). the product's materials (physical relationship, kg).
Besides, the energy consumption in the specific steps
The composed datasets for this project are representative and only used for MICROTHERM® Flexible panels range,
relevant for MICROTHERM® Flexible panels range produced has been added to the energy consumption.
by MICROTHERM® in Sint-Niklaas. • Only facility level data were available for the production
waste and the packaging of the final product. The
Data are as much as possible representative for the modern production waste has been allocated to the individual
state-of-technology. As such, the period post 2008 is product using the annual production volume of the
considered as the time coverage for the life cycle inventory products materials (physical relationship, kg).
data. The data collected by MICROTHERM® are based on data
3.10 Comparability
from the year 2021.
Basically, a comparison or an evaluation of EPD data is only
The MICROTHERM® plant in Sint-Niklaas purchases possible if all the data sets to be compared were created
hydropower from Norway, so the electricity consumption has according to EN 15804 and the building context, respectively
been modelled using the Ecoinvent 3.8 datarecord 'Electricity, the product-specific characteristics of performance, are taken
high voltage {NO}| electricity production, hydro, reservoir, alpine into account. Ecoinvent 3.8 and Industry 2.0
region | Cut-off, U'.
4. LCA: Scenarios and additional technical information
End of life (C1 - C4)
Characteristic product properties biogenic carbon
100% landfill scenario is considered as the average European
The product does not contain biogenic carbon. Its
scenario for flexible panels.
accompanying packaging contains biogenic carbon in the form
of wooden pallets, core boards and carton. Note: 1 kg of Name Value Unit
biogenic Carbon is equivalent to 44/12 kg of CO 2. Collected separately waste type - kg
Information on describing the biogenic Carbon Content at Collected as mixed construction waste 2.2 kg
factory gate Reuse - kg
Name ValueUnit Recycling - kg
kg Energy recovery - kg
Biogenic carbon content in product -
C Landfilling 2.2 kg
Biogenic carbon content in accompanying kg
0.139 Reuse, recovery and/or recycling potentials (D), relevant
packaging C
scenario information
No benefits and loads regarding the product are allocated to
module D, as the product is 100 % landfilled. However, some
Installation into the building (A5) minor benefits and loads regarding the packaging of the
Only packaging waste is included in module A5. As different product are allocated to module D.
applications and installation scenarios can be applied, the Name Value Unit
installation scenario itself is not included.
Name Value Unit
Environmental-Product Declaration - ETEX - MICROTHERM® Flexible panels range: (Semi-)Overstitched Panels, (Semi-)Quilted Panels, Slatted Panels, Aeroguard
4 (>160 kg/m3) and Slimflex
5. LCA: Results
DESCRIPTION OF THE SYSTEM BOUNDARY (X = INCLUDED IN LCA; ND = MODULE OR INDICATOR NOT DECLARED; MNR =
MODULE NOT RELEVANT)
Benefits and
Construction loads beyond
Product stage Use stage End of life stage
process stage the system
boundaries
la ire ta m w a Ry lp p u s tro p s n a rT g n iru tc a fu n a M e h t m o rf tro p s n a rTe tis e h t o t e ta g y lb m e s s A e s U e c n a n e tn ia M ria p e R tn e m e c a lp e R tn e m h s ib ru fe R y g re n e la n o ita re p Oe s u re ta w la n o ita re p Oe s u n o itc u rts n o c -e Dn o itilo m e d tro p s n a rT g n is s e c o rp e ts a W la s o p s iD -e s u e R-y re v o c e R-g n ilc y c e Rla itn e to p
A1 A2 A3 A4 A5 B1 B2 B3 B4 B5 B6 B7 C1 C2 C3 C4 D
X X X MND X MND MND MNR MNR MNR MND MND MND X X X X
RESULTS OF THE LCA - ENVIRONMENTAL IMPACT according to EN 15804+A2: 1 m^2 MICROTHERM Flexible panel
Parameter Unit A1-A3 A5 C2 C3 C4 D
Global Warming Potential total (GWP-total) kg CO 2 eq 7.99E+00 5.58E-01 2.87E-02 0 1.34E-02 -3.76E-01
Global Warming Potential fossil fuels (GWP-fossil) kg CO 2 eq 8.32E+00 7.91E-02 2.87E-02 0 1.33E-02 -1.89E-01
Global Warming Potential biogenic (GWP-biogenic) kg CO 2 eq -3.81E-01 4.78E-01 1.03E-05 0 2.53E-05 -1.87E-01
Global Warming Potential luluc (GWP-luluc) kg CO 2 eq 5.08E-02 4.61E-06 1.15E-05 0 9.84E-06 -3.3E-04
Depletion potential of the stratospheric ozone layer (ODP) kg CFC11 eq 2.07E-06 2.51E-09 6.64E-09 0 4.94E-09 -1.46E-08
Acidification potential of land and water (AP) mol H+ eq 4.61E-02 7.53E-05 8.14E-05 0 1.18E-04 -6.55E-04
Eutrophication potential aquatic freshwater (EP-freshwater) kg P eq 5.87E-04 1.23E-07 2.04E-07 0 4.09E-07 -7.33E-06
Eutrophication potential aquatic marine (EP-marine) kg N eq 1.8E-02 3.15E-05 1.62E-05 0 4.02E-05 -1.26E-04
Eutrophication potential terrestrial (EP-terrestrial) mol N eq 1.02E-01 3.12E-04 1.8E-04 0 4.44E-04 -1.41E-03
Formation potential of tropospheric ozone photochemical oxidants kg NMVOC
2.55E-02 9.26E-05 6.93E-05 0 1.26E-04 -5.57E-04
(POCP) eq
Abiotic depletion potential for non fossil resources (ADPE) kg Sb eq 6.11E-05 2.92E-08 7.76E-08 0 3.16E-08 -5.8E-07
Abiotic depletion potential for fossil resources (ADPF) MJ 1.39E+02 1.74E-01 4.35E-01 0 3.81E-01 -4.83E+00
m3 world eq
Water use (WDP) 1.61E+01 9.9E-04 1.32E-03 0 1.78E-03 -8.77E-02
deprived
RESULTS OF THE LCA - INDICATORS TO DESCRIBE RESOURCE USE according to EN 15804+A2: 1 m^2 MICROTHERM
Flexible panel
Parameter Unit A1-A3 A5 C2 C3 C4 D
Renewable primary energy as energy carrier (PERE) MJ 2.21E+01 1.37E+00 6.11E-03 0 1.97E-02 0
Renewable primary energy resources as material utilization
MJ 4.36E+00 -2.75E+00 0 0 0 2.8E+00
(PERM)
Total use of renewable primary energy resources (PERT) MJ 2.65E+01 -1.38E+00 6.11E-03 0 1.97E-02 2.8E+00
Non renewable primary energy as energy carrier (PENRE) MJ 1.57E+02 1.09E+00 4.37E-01 0 3.91E-01 0
Non renewable primary energy as material utilization (PENRM) MJ 2.86E+00 -1.75E+00 0 0 0 8.33E-01
Total use of non renewable primary energy resources (PENRT) MJ 1.6E+02 -6.52E-01 4.37E-01 0 3.91E-01 8.33E-01
Use of secondary material (SM) kg 0 0 0 0 0 3.08E-01
Use of renewable secondary fuels (RSF) MJ 0 0 0 0 0 0
Use of non renewable secondary fuels (NRSF) MJ 0 0 0 0 0 0
Use of net fresh water (FW) m3 3.88E-01 1.08E-04 3.2E-05 0 4.1E-04 -1.92E-03
RESULTS OF THE LCA – WASTE CATEGORIES AND OUTPUT FLOWS according to EN 15804+A2:
1 m^2 MICROTHERM Flexible panel
Parameter Unit A1-A3 A5 C2 C3 C4 D
Hazardous waste disposed (HWD) kg 1.31E-04 4.13E-07 1.13E-06 0 4.18E-07 -2.83E-06
Non hazardous waste disposed (NHWD) kg 1.27E+00 1.51E-01 2.28E-02 0 2.2E+00 -1E-02
Radioactive waste disposed (RWD) kg 5.37E-04 1.12E-06 2.94E-06 0 2.6E-06 -9.63E-06
Components for re-use (CRU) kg 0 0 0 0 0 0
Materials for recycling (MFR) kg 1.9E-01 1.17E-01 0 0 0 -3.08E-01
Materials for energy recovery (MER) kg 0 0 0 0 0 0
Exported electrical energy (EEE) MJ 3.26E-02 2.28E-01 0 0 0 -2.6E-01
Exported thermal energy (EET) MJ 6.52E-02 4.55E-01 0 0 0 -5.21E-01
RESULTS OF THE LCA – additional impact categories according to EN 15804+A2-optional:
1 m^2 MICROTHERM Flexible panel
Parameter Unit A1-A3 A5 C2 C3 C4 D
Disease
Incidence of disease due to PM emissions (PM) 4.81E-07 1.27E-09 2.3E-09 0 2.28E-09 -7.93E-09
incidence
Human exposure efficiency relative to U235 (IR) kBq U235 eq 5.03E-01 7.65E-04 1.89E-03 0 1.95E-03 -1.07E-02
Comparative toxic unit for ecosystems (ETP-fw) CTUe 5.99E+02 1.65E-01 3.41E-01 0 2.19E-01 -1.17E+00
Comparative toxic unit for humans (carcinogenic) (HTP-c) CTUh 7.06E-09 4.08E-11 1.1E-11 0 6.35E-12 -5.89E-11
Environmental-Product Declaration - ETEX - MICROTHERM® Flexible panels range: (Semi-)Overstitched Panels, (Semi-)Quilted Panels, Slatted Panels, Aeroguard
5 (>160 kg/m3) and Slimflex
Comparative toxic unit for humans (noncarcinogenic) (HTP-nc) CTUh 7.08E-07 2.72E-10 3.45E-10 0 1.29E-10 -1.37E-09
Soil quality index (SQP) SQP 1.65E+02 1.76E-01 3.03E-01 0 7.19E-01 -2.14E+01
Disclaimer 1 – for the indicator “Potential Human exposure efficiency relative to U235”. This impact category deals mainly with the
eventual impact of low-dose ionizing radiation on human health of the nuclear fuel cycle. It does not consider effects due to possible
nuclear accidents, occupational exposure nor due to radioactive waste disposal in underground facilities. Potential ionizing radiation
from the soil, from radon and from some construction materials is also not measured by this indicator.
Disclaimer 2 – for the indicators “abiotic depletion potential for non-fossil resources”, “abiotic depletion potential for fossil resources”,
“water (user) deprivation potential, deprivation-weighted water consumption”, “potential comparative toxic unit for ecosystems”,
“potential comparative toxic unit for humans – cancerogenic”, “Potential comparative toxic unit for humans - not cancerogenic”,
“potential soil quality index”. The results of this environmental impact indicator shall be used with care as the uncertainties on these
results are high or as there is limited experienced with the indicator.
6. LCA: Interpretation
For MICROTHERM® Flexible panels produced in Belgium, the second most important life cycle stage (i.e. energy
raw materials used in the formulation mix has the highest consumption), but far less than the raw materials. Module D is
contribution on all impact categories, and more specific the not significant as the product is not recycled nor incinerated.
fumed silica and fumed alumina. Also, the manufacturing is the
7. Requisite evidence
No evidence is required
8. References
Standards range of Environmental Product Declarations of Institute
Construction and Environment e.V. (IBU) : Requirements on the
EN15804 EPD for Mineral insulating materials
EN 15804:2012+A2:2019+AC:2021, Sustainability of
construction works — Environmental Product Declarations — Further references
Core rules for the product category of construction products.
Biocide Products No. 528/2012
EN16757 EU, REGULATION (EU) No 528/2012 OF THE
EN 16757:2017, Sustainability of construction works– EUROPEANPARLIAMENT
Environmental product declarations – Product Category Rules
for concrete and concrete elements CPR
European Regulation N° 305/2011 (CPR)
ISO 9001
ISO 9001:2015: Quality management systems — Requirements Ecoinvent
Wernet, G., Bauer, C., Steubing, B., Reinhard, J., Moreno-Ruiz,
ISO 14001 E., and Weidema, B., 2016. The ecoinvent database version 3
ISO 14001:2015: Environmental management systems — (part I): overview and methodology. The International Journal of
Requirements with guidance for use Life Cycle Assessment, [online] 21(9), pp.1218–1230. Available
at:http://link.springer.com/10.1007/s11367-016-1087-
ISO 14025 8.
EN ISO 14025:2011, Environmental labels and declarations —
Type III environmental declarations — Principles and Enperas Quadrant tool. 2022. Genk, Belgium.
procedures.
IBU
ISO 14040 IBU 2021. Institut Bauen und Umwelt e.V.: General Instructions
ISO 14040:2006: Environmental management – Life cycle for the EPD programme of Institut Bauen und Umwelt e.V.,
assessment – Principles and framework. Version 2.0, Berlin: Institut Bauen und Umwelt e.V., 2021
www.ibu-epd.com
ISO 14044
ISO 14044:2006: Environmental management – Life cycle Industry 2.0
assessment – Requirements and guidelines. Industry 2.0 (from PlasticsEurope, worldsteel and ERASM).
LCA database as integrated in SimaPro 9.3.0.3.
ISO 45001
ISO 45001:2018: Occupational health and safety management PEFCR
systems Requirements with guidance for use European commission (2018). Product Environmental Footprint
Category Rules PEFCR Guidance, version 6.3.
PCR Part A
Calculation rules for the Life Cycle Assessment and Pré Consultants (2021) SimaPro 9.2.0.1 [Computer Software].
Requirements on the Background Report, Institut Bauen und Amersfoort, The Netherlands.
Umwelt e.V., www.bauumwelt.com.
REACH candidate list
PCR Part B ECHA, REACH Candidate List of substances of very
Institut Bauen und Umwelt e.V, Berlin (pub.): PCR Guidance- highconcern for Authorisation
Texts for Building-Related Products and Services From the
Environmental-Product Declaration - ETEX - MICROTHERM® Flexible panels range: (Semi-)Overstitched Panels, (Semi-)Quilted Panels, Slatted Panels, Aeroguard
6 (>160 kg/m3) and Slimflex
The literature referred to in the Environmental Product The current version of PCR Part A and PCR Part B of the PCR
Declaration must be listed in full.Standards already fully quoted document on which they are based must be referenced.
in the EPD do not need to be listed here again.
Environmental-Product Declaration - ETEX - MICROTHERM® Flexible panels range: (Semi-)Overstitched Panels, (Semi-)Quilted Panels, Slatted Panels, Aeroguard
7 (>160 kg/m3) and Slimflex
Publisher
Institut Bauen und Umwelt e.V. +49 (0)30 3087748- 0
Hegelplatz 1 info@ibu-epd.com
10117 Berlin www.ibu-epd.com
Germany
Programme holder
Institut Bauen und Umwelt e.V. +49 (0)30 3087748- 0
Hegelplatz 1 info@ibu-epd.com
10117 Berlin www.ibu-epd.com
Germany
Author of the Life Cycle Assessment
Owner of the Declaration
Etex Building Performance International +32 2 778 12 11
Rue Marcel Demonque 500 info@etexgroup.com
84915 Avignon Cedex 9 www.etexgroup.com
France
Environmental-Product Declaration - ETEX - MICROTHERM® Flexible panels range: (Semi-)Overstitched Panels, (Semi-)Quilted Panels, Slatted Panels, Aeroguard
8 (>160 kg/m3) and Slimflex
