ENVIRONMENTAL PRODUCT DECLARATION
as per ISO 14025 and EN 15804+A2
Owner of the Declaration dormakaba International Holding GmbH
Publisher Institut Bauen und Umwelt e.V. (IBU)
Programme holder Institut Bauen und Umwelt e.V. (IBU)
Declaration number EPD-DOR-20210339-CBA2-EN
Issue date 04.05.2022
Valid to 03.05.2027
c-lever compact
dormakaba
www.ibu-epd.com | https://epd-online.com
General Information
dormakaba c-lever compact
Programme holder Owner of the declaration
IBU – Institut Bauen und Umwelt e.V. dormakaba International Holding GmbH
Hegelplatz 1 DORMA Platz 1
10117 Berlin 58256 Ennepetal
Germany Germany
Declaration number Declared product / declared unit
EPD-DOR-20210339-CBA2-EN 1 piece of the product: c-lever pro
This declaration is based on the product category rules: Scope:
Building Hardware products, 01.08.2021 This EPD refers to a specific product manufactured by dormakaba. The
(PCR checked and approved by the SVR) production site is located in Shenzhen (China).
The data represent the year 2020.
Issue date The owner of the declaration shall be liable for the underlying information
and evidence; the IBU shall not be liable with respect to manufacturer
04.05.2022
information, life cycle assessment data and evidences.
The EPD was created according to the specifications of EN 15804+A2. In
Valid to
the following, the standard will be simplified as EN 15804.
03.05.2027
Verification
The standard EN 15804 serves as the core PCR
Independent verification of the declaration and data according to ISO
14025:2011
internally X externally
Dipl.-Ing. Hans Peters
(Chairman of Institut Bauen und Umwelt e.V.)
Florian Pronold Dr.-Ing. Wolfram Trinius,
(Managing Director Institut Bauen und Umwelt e.V.) (Independent verifier)
1 Environmental Product Declaration - dormakaba - c-lever compact
Product
Power supply
Product description/Product definition
The electronic fitting c-lever compact combines design and - 2 batteries 1.5 V AAA L92, FR3
functionality. The access medium can be determined according
to individual needs - cards, key fobs, keys with Radio The products are not harmonised in accordance with the
Frequency Identification (RFID) or smartphones. Access rights Construction Product Regulations (CPR) but in accordance with
can be defined for an almost unlimited number of users, other provisions for harmonisation of the EU.
precisely to the location and time. These can be changed Compliance with the European Union Directive and technical
flexibly, either in standalone or wireless operation. The c-lever specifications:
compact can be integrated into all dormakaba system solutions
• EN 300328 V2.1.1:2016-11
and supports the latest RFID technologies. With the selectable
• EN 300330 V2.1.1: 2017-02
wireless function you transmit your access rights from your PC
• EN 301489-1 V2.2:2017-03
to the door components via radio. Benefit from the advantages
• EN 301489-3 V2.2:2017-03
in terms of security, programming and maintenance. For the
• EN 301489-17 V3.1.1:2017-07
placing on the market in the European Union/European Free
• EN 50364:2010
Trade Association (EU/EFTA) (with the exception of
• EN 60529:2014-09
Switzerland) the following legal provisions apply:
The provisions of the Radio Equipment Directive (RED) are
• EN 301489:2017 met. The products are subject to CE marking according to the
• EN 300330:2017 relevant harmonization legislation.
• Radio Equipment Directive (RED)
• Restriction of Hazardous Substances (RoHS) Base materials/Ancillary materials
The CE-marking considers the proof of conformity with the The major material compositions including the packaging of the
respective harmonized standards based on the legal provisions product are listed below:
above. For the application and use the respective national Name Value Unit
provisions apply.
Steel 35 %
Application Paper 26 %
The c-lever compact is a mechatronical door fitting which does Zinc 16 %
not require any additional cabling and offer a fully wireless, Stainless steel 15 %
network-compatible electronic locking solution with a range of
Plastics 5 %
functions.
Electronics 3 %
Possible fields of application are:
Others <1 %
• Interior doors - wooden, metal and glass doors
The product includes partial articles which contain substances
Technical Data listed in the Candidate List of REACH Regulation
The c-lever compact has the following technical properties: 1907/2006/EC (date: 17.01.2022) exceeding 0.1 percentage by
Name Value Unit mass: yes
54,7 x 122,8 x
Dimensions (W X H x D) mm - Lead (Pb): 7439-92-1 (CAS-No.) is included in some of the
21,9
alloys used. The concentration of lead in each individual alloy
Temperature -25 to +70 °C
does not exceed 4.0% (by mass).
Protection class IP54
Humidity non-corresponding 0 to 95 % The Candidate List can be found on the ECHA website
up to 60,000 or up to 3 address: https:echa.europa.eu/de/home.
Battery life at 20 °C
cylces years
Weight (without packaging) 0,94 kg
Reference service life
Weight (with packaging) 1,27 kg
The product is certified according to EN 1906 and EN 16867 for
Power consumption "on mode" 0,00009 W 250.000 cycles. Under normal conditions and depending on
Power consumption "standby cycle frequency, door weight etc., it means an approximate
0,00009 W
mode" duration of 10 years.
LCA: Calculation rules
The following modules are declared: A1-A3, C, D and additional
Declared Unit modules: A4 + A5 + B6
The declared unit is 1 piece of the product: c-lever compact.
Declared unit Production - Module A1-A3
The product stage includes:
Name Value Unit
— A1, raw material extraction, processing of secondary
Declared unit 1 piece/product
material input (e.g. recycling processes),
Mass 1.28 kg — A2, transport to the manufacturer,
— A3, manufacturing and assembly, processing and
System boundary mechanical treatments, including provision of all materials,
The type of EPD is according to EN 15804: "cradle to gate with products and energy, as well as waste processing up to the
options, modules C1–C4, and module D". end-of waste state.
2 Environmental Product Declaration - dormakaba - c-lever compact
Construction stage - Modules A4-A5 Module D (Benefits and loads beyond the system boundary)
The construction process stage includes: includes:
— A4, transport to the building site; — D, recycling potentials, expressed as net impacts and
— A5, treatment of waste packaging materials arising during benefits.
installation into the building.
Geographic Representativeness
Use stage - Module B6 Land or region, in which the declared product system is
The use stage related to the operation of the building includes: manufactured, used or handled at the end of the product´s
— B6, operational energy use lifespan: China
End-of-life stage– Modules C1-C4 and D
Comparability
The end-of-life stage includes:
Basically, a comparison or an evaluation of EPD data is only
— C1, de-construction, demolition:
possible if all the data sets to be compared were created
— C2, transport to waste processing;
according to EN 15804 and the building context, respectively
— C3, waste processing for reuse, recovery and/or recycling;
the product-specific characteristics of performance, are taken
— C4, disposal;
into account. Background database: GaBi, SP40.
including provision and all transport, provision of all materials,
products and related energy and water use.
LCA: Scenarios and additional technical information
Name Value Unit
Characteristic product properties of biogenic carbon
Life Span according to the manufacturer 10 a
Information on describing the biogenic Carbon Content at
factory gate Operational energy use (B6)
Name ValueUnit The use stage is declared for 10 years.
Biogenic carbon content in accompanying kg Name Value Unit
0.12
packaging C Electricity consumption for 1 year 0,003 kWh
Note: 1 kg of biogenic carbon is equivalent to 44/12 kg of CO . Days per year in use 365 days
2
Power consumption "on mode" 0,06 W
Hours per day in use "on mode" 0,1 h
The following technical scenario information is required for the Power consumption "standby mode" 0,00009 W
declared modules.
Hours per day in use "standby mode" 23,9 h
Transport to the building site (A4)
End of life (C1-C4)
Name Value Unit
C1: The product dismantling from the building is done manually
Litres of fuel per 1 kg (truck) 0.00276 l/100km
without environmental burden.
Transport distance (truck) 1000 km
Name Value Unit
Capacity utilisation (including empty runs) 51 %
Collected separately waste type 0.95 kg
Transport distance (ship) 20300 km
Recycling 0.86 kg
Installation into the building (A5) Energy recovery 0.05 kg
Name Value Unit Final deposition 0,03 kg
Waste packaging (paper) 0.32 kg Reuse, recovery and/or recycling potentials (D), relevant
Waste packaging (plastic) 0,005 kg scenario information
Collection rate is 100%
Reference service life
3 Environmental Product Declaration - dormakaba - c-lever compact
LCA: Results
DESCRIPTION OF THE SYSTEM BOUNDARY (X = INCLUDED IN LCA; MND = MODULE OR INDICATOR NOT DECLARED; MNR
= MODULE NOT RELEVANT)
Benefits and
Construction loads beyond
Product stage Use stage End of life stage
process stage the system
boundaries
la ire ta m w a Ry lp p u s tro p s n a rT g n iru tc a fu n a M e h t m o rf tro p s n a rTe tis e h t o t e ta g y lb m e s s A e s U e c n a n e tn ia M ria p e R tn e m e c a lp e R tn e m h s ib ru fe R y g re n e la n o ita re p Oe s u re ta w la n o ita re p Oe s u n o itc u rts n o c -e Dn o itilo m e d tro p s n a rT g n is s e c o rp e ts a W la s o p s iD -e s u e R-y re v o c e R-g n ilc y c e Rla itn e to p
A1 A2 A3 A4 A5 B1 B2 B3 B4 B5 B6 B7 C1 C2 C3 C4 D
X X X X X MND MND MNR MNR MNR X MND X X X X X
RESULTS OF THE LCA - ENVIRONMENTAL IMPACT according to EN 15804+A2: 1 piece c-lever compact
Parameter Unit A1-A3 A4 A5 B6 C1 C2 C3 C4 D
GWP-total kg CO 2 eq 1.24E+01 1.97E-01 4.73E-01 1.1E-02 0 4E-03 1.38E-01 4.84E-04 -2.57E+00
GWP-fossil kg CO 2 eq 1.27E+01 1.92E-01 2.4E-02 1.1E-02 0 4E-03 1.38E-01 4.81E-04 -2.57E+00
GWP-biogenic kg CO 2 eq -3.24E-01 5E-03 4.49E-01 3.39E-05 0 1.83E-04 3.22E-06 1.65E-06 6.45E-04
GWP-luluc kg CO 2 eq 8.13E-03 4.3E-06 8.29E-06 1.54E-05 0 9.43E-08 7.82E-06 1.39E-06 -2E-03
ODP kg CFC11 eq 1.29E-10 1.93E-17 8.93E-17 2.26E-16 0 4.18E-19 6.97E-17 1.79E-18 -7.23E-15
AP mol H+ eq 5.4E-02 3E-03 1.31E-04 2.76E-05 0 3.97E-06 2.46E-05 3.45E-06 -1.6E-02
EP-freshwater kg P eq 2.22E-05 4.2E-08 1.72E-08 2.75E-08 0 8.48E-10 1.11E-08 8.27E-10 -3.25E-06
EP-marine kg N eq 1.3E-02 8.6E-04 4.7E-05 5.78E-06 0 1.26E-06 5.55E-06 8.89E-07 -2E-03
EP-terrestrial mol N eq 1.45E-01 9E-03 5.9E-04 6.11E-05 0 1.4E-05 1.12E-04 9.77E-06 -2.3E-02
kg NMVOC
POCP 3.8E-02 2E-03 1.25E-04 1.6E-05 0 3.57E-06 1.54E-05 2.69E-06 -7E-03
eq
ADPE kg Sb eq 1.02E-03 5.39E-09 1.4E-09 2.99E-09 0 1.19E-10 9.57E-10 4.32E-11 -6.2E-04
ADPF MJ 1.67E+02 2.55E+00 1.51E-01 1.86E-01 0 5.6E-02 6.4E-02 6E-03 -3.06E+01
m3 world eq
WDP 2.97E+00 3.62E-04 5.8E-02 2E-03 0 7.77E-06 1.4E-02 5.05E-05 -5.96E-01
deprived
GWP = Global warming potential; ODP = Depletion potential of the stratospheric ozone layer; AP = Acidification potential of land and water; EP =
Eutrophication potential; POCP = Formation potential of tropospheric ozone photochemical oxidants; ADPE = Abiotic depletion potential for non-fossil
resources; ADPF = Abiotic depletion potential for fossil resources; WDP = Water (user) deprivation potential)
RESULTS OF THE LCA - INDICATORS TO DESCRIBE RESOURCE USE according to EN 15804+A2: 1 piece c-lever compact
Parameter Unit A1-A3 A4 A5 B6 C1 C2 C3 C4 D
PERE MJ 2.55E+01 8E-03 3.92E+00 8E-02 0 1.77E-04 1.7E-02 8.27E-04 -4.8E+00
PERM MJ 3.89E+00 0 -3.89E+00 0 0 0 0 0 0
PERT MJ 2.94E+01 8E-03 2.8E-02 8E-02 0 1.77E-04 1.7E-02 8.27E-04 -4.8E+00
PENRE MJ 1.65E+02 2.55E+00 3.66E-01 1.86E-01 0 5.6E-02 2.12E+00 6E-03 -3.06E+01
PENRM MJ 2.27E+00 0 -2.15E-01 0 0 0 -2.06E+00 0 0
PENRT MJ 1.67E+02 2.55E+00 1.51E-01 1.86E-01 0 5.6E-02 6.4E-02 6E-03 -3.06E+01
SM kg 3.22E-01 0 0 0 0 0 0 0 0
RSF MJ 0 0 0 0 0 0 0 0 0
NRSF MJ 0 0 0 0 0 0 0 0 0
FW m3 8.14E-02 1.47E-05 1E-03 9.54E-05 0 3.18E-07 3.38E-04 1.59E-06 -2.1E-02
PERE = Use of renewable primary energy excluding renewable primary energy resources used as raw materials; PERM = Use of renewable primary
energy resources used as raw materials; PERT = Total use of renewable primary energy resources; PENRE = Use of non-renewable primary energy
excluding non-renewable primary energy resources used as raw materials; PENRM = Use of non-renewable primary energy resources used as raw
materials; PENRT = Total use of non-renewable primary energy resources; SM = Use of secondary material; RSF = Use of renewable secondary fuels;
NRSF = Use of non-renewable secondary fuels; FW = Use of net fresh water
RESULTS OF THE LCA – WASTE CATEGORIES AND OUTPUT FLOWS according to EN 15804+A2:
1 piece c-lever compact
Parameter Unit A1-A3 A4 A5 B6 C1 C2 C3 C4 D
HWD kg 3.39E-06 2.49E-10 2.37E-10 7.75E-11 0 5.46E-12 2.44E-10 9.63E-11 -7.37E-07
NHWD kg 3.18E-01 2.61E-04 1.6E-02 1.29E-04 0 5.75E-06 1.4E-02 3.2E-02 -3.1E-02
RWD kg 3.56E-03 2.78E-06 7.85E-06 2.72E-05 0 6.04E-08 2.38E-06 7.19E-08 -8.33E-04
CRU kg 0 0 0 0 0 0 0 0 0
MFR kg 0 0 0 0 0 0 8.62E-01 0 0
MER kg 0 0 0 0 0 0 0 0 0
EEE MJ 1.42E-01 0 7.2E-01 0 0 0 0 0 0
EET MJ 2.57E-01 0 1.32E+00 0 0 0 0 0 0
HWD = Hazardous waste disposed; NHWD = Non-hazardous waste disposed; RWD = Radioactive waste disposed; CRU = Components for re-use;
MFR = Materials for recycling; MER = Materials for energy recovery; EEE = Exported electrical energy; EET = Exported thermal energy
4 Environmental Product Declaration - dormakaba - c-lever compact
RESULTS OF THE LCA – additional impact categories according to EN 15804+A2-optional:
1 piece c-lever compact
Parameter Unit A1-A3 A4 A5 B6 C1 C2 C3 C4 D
Disease
PM 4.89E-07 5.4E-08 7.43E-10 2.67E-10 0 2.09E-11 3.14E-10 4.27E-11 -2E-07
incidence
IR kBq U235 eq 3.43E-01 3.98E-04 1E-03 4E-03 0 8.63E-06 2.14E-04 7.4E-06 -9.7E-02
ETP-fw CTUe 1.01E+02 1.8E+00 7.1E-02 7.8E-02 0 4E-02 2.4E-02 4E-03 -1.09E+01
HTP-c CTUh 2.81E-07 3.39E-11 3.84E-12 2.22E-12 0 7.49E-13 2.08E-12 5.35E-13 9.04E-10
HTP-nc CTUh 2.85E-07 1.52E-09 1.77E-10 8.27E-11 0 3.2E-11 2.11E-10 5.89E-11 2.96E-07
SQP SQP 8.59E+01 7E-03 4E-02 5.8E-02 0 1.44E-04 1.9E-02 1E-03 -2.64E+00
PM = Potential incidence of disease due to PM emissions; IR = Potential Human exposure efficiency relative to U235; ETP-fw = Potential comparative
Toxic Unit for ecosystems; HTP-c = Potential comparative Toxic Unit for humans (cancerogenic); HTP-nc = Potential comparative Toxic Unit for humans
(not cancerogenic); SQP = Potential soil quality index
Disclaimer 1 – for the indicator IRP
This impact category deals mainly with the eventual impact of low dose ionizing radiation on human health of the nuclear fuel cycle. It
does not consider effects due to possible nuclear accidents, occupational exposure nor due to radioactive waste disposal in
underground facilities. Potential ionizing radiation from the soil, from radon and from some construction materials is also not measured
by this indicator.
Disclaimer 2 – for the indicators ADPE, ADPF, WDP, ETP-fw, HTP-c, HTP-nc, SQP
The results of this environmental impact indicator shall be used with care as the uncertainties on these results are high or as there is
limited experience with the indicator.
References
Standards (EMC) standard for radio equipment and services - Part 3:
Specific conditions for Short-Range Devices (SRD) operating
EN 1906 on frequencies between 9 kHz and 246 GHz - Harmonised
EN 1906:2012, Building hardware - Lever handles and knob Standard covering the essential requirements ofarticle 3.1(b) of
furniture - Requirements and test methods; German version EN Directive 2014/53/EU.
1906:2012.
EN 301489-17 V3.1.1
EN 16867 EN 301489-17 V3.1.1:2017-07, ElectroMagnetic Compatibility
EN 16867:2020, Building hardware - Mechatronic door (EMC) standard for radio equipment and services - Part 17:
furniture - Requirements and test methods; German version EN Specific conditions for Broadband Data Transmission Systems -
16867:2020. Harmonised Standard covering the essential requirements of
article 3.1(b) of Directive 2014/53/EU.
EN 15804+A2
EN15804:2019+A2, Sustainability of construction works — EN 50364
Environmental Product Declarations — Core rules for the EN 50364:2010, Limitation of human exposure to
product category of construction products. electromagnetic fields from devices operating in the frequency
range 0 Hz to 300 GHz, used in Electronic Article Surveillance
EN 300328 V2.1.1 (EAS), Radio Frequency Identification (RFID) and similar
EN 300328 V2.1.1;2016-11, Wideband transmission systems - applications.
Data transmission equipment operating in the 2,4 GHz ISM
band and using wide band modulation techniques - EN 60529
Harmonised Standard covering the essential requirements of EN 60529:2014-09, Degrees of protection provided by
article 3.2 of the Directive 2014/53/EU. enclosures (IP Code, IEC 60529:1989 + A1:1999 + A2:2013).
EN 300330 V2.1.1 ISO 14025
EN 300330 V2.1.1:2017-02, Short Range Devices (SRD) - DIN EN ISO 14025:2011-10, Environmental labels and
Radio equipment in the frequency range 9 kHz to 25 MHz and declarations — Type III environmental declarations —
inductive loop systems in the frequency range 9 kHz to 30 Principles and procedures.
MHz - Harmonised Standard covering the essential
requirements of article 3.2 of the Directive 2014/53/EU Radio Equipment Directive (RED)
(Endorsement of the English version EN 300 330 V2.1.1 (2017- Directive 2014/53/EU of the European Parliament and of the
02) as German standard). Council of 16 April 2014 on the harmonisation of the laws of the
Member States relating to the making available on the market
EN 301489-1 V2.2 of radio equipment and repealing Directive 1999/5/EC.
EN 301489-1 V2.2:2017-03, ElectroMagnetic Compatibility
(EMC) standard for radio equipment and services - Part 1: Registration, Evaluation, Authorisation and Restriction of
Common technical requirements - Harmonised Standard Chemicals (REACH)
covering the essential requirements of article 3.1(b) of Directive Regulation (EC) No 1907/2006 of the European Parliament and
2014/53/EU and the essential requirements of article 6 of of the Council on the Registration, Evaluation, Authorisation
Directive 2014/30/EU. and Restriction of Chemicals (REACH).
EN 301489-3 V2.2 Restriction of Hazardous Substances (RoHS)
EN 301489-3 V2.2:2017-03, Electromagnetic compatibility and Directive on the restriction of the use of certain hazardous
Radio spectrum Matters (ERM) - ElectroMagnetic Compatibility substances in electrical and electronic equipment (RoHS),
5 Environmental Product Declaration - dormakaba - c-lever compact
Directive (EU) No 2011/65. documentation/).
Further References LCA-tool dormakaba
LCA-tool, IBU-DOR-202101-LT1-EN.
IBU 2021 Developed by Sphera Solutions GmbH.
Institut Bauen und Umwelt e.V.: General Instructions for the
EPDs programme of Institut Bauen und Umwelt e.V. Version PCR Part A
2.0., Berlin: Institut Bauen und Umwelt e.V., 2021. www.ibu- PCR – Part A: Calculation Rules for the Life Cycle As-sessment
epd.com and Requirements on the Project Re-port according to EN
GaBi ts software 15804+A2:2019, Version 1.0, Institut Bauen und Umwelt e.V.,
Sphera Solutions GmbH Gabi Software System and Database www.ibu-epd.com.
for Life Cycle Engineering 1992-2020 Version 10.0.0.71
University of Stuttgart Leinfelden-Echterdingen PCR Part B
PCR – Part B: Requirements on the EPD for Building Hardware
GaBi ts documentation product, version 1.2, Institut Bauen und Umwelt e.V., www.ibu-
GaBi life cycle inventory data documentation (https://www.gabi- epd.com, 2017.
software.com/support/gabi/gabi-database-2020-lci-
6 Environmental Product Declaration - dormakaba - c-lever compact
Publisher
Institut Bauen und Umwelt e.V. +49 (0)30 3087748- 0
Hegelplatz 1 info@ibu-epd.com
10117 Berlin www.ibu-epd.com
Germany
Programme holder
Institut Bauen und Umwelt e.V. +49 (0)30 3087748- 0
Hegelplatz 1 info@ibu-epd.com
10117 Berlin www.ibu-epd.com
Germany
Author of the Life Cycle Assessment
Sphera Solutions GmbH +49 711 341817-0
Hauptstraße 111- 113 info@sphera.com
70771 Leinfelden-Echterdingen www.sphera.com
Germany
Owner of the Declaration
dormakaba International Holding GmbH +49 2333 793-0
DORMA Platz 1 info.de@dormakaba.com
58256 Ennepetal www.dormakaba.com
Germany
7 Environmental Product Declaration - dormakaba - c-lever compact
