ENVIRONMENTAL PRODUCT DECLARATION
as per ISO 14025 and EN 15804+A2
Owner of the Declaration VELUX Group
Publisher Institut Bauen und Umwelt e.V. (IBU)
Programme holder Institut Bauen und Umwelt e.V. (IBU)
Declaration number EPD-VEL-20220138-IBJ3-EN
Issue date 25.07.2022
Valid to 24.07.2027
VELUX flat roof window CVP - grid-connected
VELUX A/S
www.ibu-epd.com | https://epd-online.com
1. General Information
VELUX A/S VELUX flat roof window CVP - grid-connected
Programme holder Owner of the declaration
IBU – Institut Bauen und Umwelt e.V. VELUX Group
Hegelplatz 1 Ådalsvej 99
10117 Berlin 2970 Hørsholm
Germany Denmark
Declaration number Declared product / declared unit
EPD-VEL-20220138-IBJ3-EN The declaration represents 1 piece of a grid-connected VELUX flat roof
window CVP Q of the size 1.20 m
x 1.20 m = 1.44 m2
This declaration is based on the product category rules: Scope:
Windows and doors , 01.08.2021 The declaration covers 100% of grid-connected VELUX flat roof windows
(PCR checked and approved by the SVR) CVP Q and CVP U by Partizánske Building Components SK, Slovenia.
The owner of the declaration shall be liable for the underlying information
and evidence; the IBU shall not be liable with respect to manufacturer
Issue date information, life cycle assessment data and evidences.
25.07.2022
The EPD was created according to the specifications of EN 15804+A2. In
the following, the standard will be simplified as EN 15804.
Valid to
Verification
24.07.2027
The standard EN 15804 serves as the core PCR
Independent verification of the declaration and data according to ISO
14025:2011
internally X externally
Dipl.-Ing. Hans Peters
(Chairman of Institut Bauen und Umwelt e.V.)
Florian Pronold Dr. Eva Schmincke,
(Managing Director Institut Bauen und Umwelt e.V.) (Independent verifier)
1 Environmental Product Declaration - VELUX A/S - VELUX flat roof window CVP - grid-connected
2. Product
and test methods.
2.1 Product description/Product definition
The grid-connected Velux flat roof windows CVP Q consist of a 2.4 Delivery status
motorised base unit made of a PVC curb with an integrated The product is available in pre-defined sizes covering 0,6x0,6m
glazing unit and hinges on one side to allow for venting. The to 1,5x1,5m.
product has insulation in 4 chambers.
The grid-connected Velux flat roof windows CVP U consist of a 2.5 Base materials/Ancillary materials
motorised base unit made of a PVC curb with integrated Composition of the base unit CVP:
glazing unit and hinges on one side to allow for venting. The PVC 40 %
product is similar to CVP Q, but with adifferent glazing unit and galvanized steel 10 %
only insulation in 2 chambers. laminated glass 25 %
tempered glass 15 %
On the of the base unit is installed a one-layer opaque or others
transparent acrylic (PMMA) dome. For the placing on the
market of the product in the European Union/European Free Composition of the top unit (ISD 0000A):
Trade Association (EU/EFTA) (with the exception of PMMA 95 %
Switzerland) Regulation (EU) No. 305/2011 (CPR) applies. The iron & cast iron 5 %
product needs a declaration of performance taking into
consideration EN 1873:2005, Prefabricated accessories for Composition of the motor (CVP):
roofing - Individual rooflights of plastics - Product specification glavanized steel 40 %
and test methods and the CE-marking. stainless steel 15 %
For the application and use the respective national provisions PSU A04 casted 10 %
apply. copper wire 10 %
DC motor 5 %
2.2 Application
Velux flat roof windows CVP are used in renovation and new 1) 'This product/article/at least one partial article contains
build. substances listed in the candidate list (date: 02.03.2022)
exceeding 0.1 percentage by mass:
2.3 Technical Data
• no
The Declaration of Performance including relevant technical
2) 'This product/article/at least one partial article contains other
specifications and test methods/test standards can be
CMR substances in categories 1A or 1B which are not on the
downloaded from the website www.velux.com/ce.
candidate list, exceeding 0.1 percentage by mass:
The declared values in the table relate to the reference product • not investigated with suppliers
incl. an average pane. For other covered product variants, 3) 'Biocide products were added to this construction product or
specific values can be selected at the bottom of the above- it has been treated with biocide products (this then concerns a
mentioned download page treated product as defined by the (EU) Regulation on Biocidal
Products No. 528/2012):
Constructional data for CVP 120120 73Q+ISD 0000
For other • no
variants, see velux.com/ce
Recycled content
Name Value Unit
Reaction to fire - class
Resistance to upward load EN 1875 UL 1500 -
water permeability acc. to EN 13985, EN
- class
1027
Resistance to downward load EN 1873 UL 2500 -
Resistance to fire EN 13501-2 NPD -
External fire performance EN 13501-5 NPD -
Water tightness EN 1873 passed - The values stated in the table relate to the recycled material
Impact resistance - small hard body passed streams in VELUX production.
passed -
EN 1873
Impact resistance - large soft body EN 1873 SB 1200 -
2.6 Manufacture
Direct airborne sound insulation EN ISO 36 (-1;- dB Base unit:
418-3 4)
Thermal transmittance EN 1873 0,80 W/(m2K) PVC profiles, gaskets, rain sensor, motor cover and wires and
Luminous transmittance EN 410 0,72 - other minor components are produced outside Velux.
Air permability EN 1026 4 Class
Motor and wall switch are assembled at production site in
Durability EN 1873 NDP -
Czech republic.
Performance data of the product in accordance with the
declaration of performance with respect to its essential The insulating glass unit is assembled at a production site in
characteristics according to France.
• EN 1873:2005, Prefabricated accessories for roofing -
Minor ABS plastic and glass fibre components are produced at
Individual rooflights of plastics - Product specification
2 Environmental Product Declaration - VELUX A/S - VELUX flat roof window CVP - grid-connected
a factory in Denmark. Health protection: According to current knowledge, no health
hazards or impairments are to be expected.
The production and final assembly of the base unit takes place
at the production site in Slovakia. 2.12 Reference service life
It is not possible to calculate the reference service life
The final production processes include preparation of the PVC according to ISO 15686. The service life based on a
frame/sash profiles by cutting, milling and drilling and manufacturer's declaration is 30 years. The corresponding
installation of EPS foam. The final PVC base is assembled by utilization scenario is declared in 4.
cutting, deburring and welding, cutting and mounting of gaskets
2.13 Extraordinary effects
and installation of the glazing unit, window opener incl. gas
springs as well as packaging, stacking and wrapping of the Fire
product on pallets.
Fire performance according to EN 13501:1
Top unit:
Name Value
Building material class B
The plastic dome is produced and assembled at a production
site in Germany. Burning droplets s1
Smoke gas development d0
The final production processes include forming/blow moulding
of the plastic dome, with afterward deburring, engraving and
Water
assembly, as well as packaging, stacking and wrapping of the
In the event of unforeseen exposure to water (flood), VELUX
product on pallets.
flat roof windows must be replaced as electrical components;
The factories are ISO 9001 certified.
no adverse effects on human health or the environment are to
be expected.
2.7 Environment and health during manufacturing
All factories are ISO 14001 and ISO 45001 certified.
Mechanical destruction
2.8 Product processing/Installation In the event of unforeseen mechanical destruction, VELUX flat
roof windows must be replaced; apart from potential injuries
The product is delivered to the customer in two parts, a top and
from glass cullet, no adverse effects on human health or the
bottom part. After the hole in the roof is prepared, the bottom
environment are to be expected.
part of the product can be installed with the use of a
screwdriver, after which the top unit can be fastened to the
2.14 Re-use phase
bottom unit.
VELUX flat roof windows can be dismantled manually without
2.9 Packaging any problems. The metal parts are usually recycled, and the
plastic parts and wood are sent for thermal recycling for energy
The packaging usually consists of:
recovery. Flat glass can be recycled whereas laminated glass is
- polyethylene film
usually used as secondary aggregate in road construction or
- polystyrene foam parts
landfilling.
- cardboard
2.15 Disposal
The use of other packaging materials is possible, but
VELUX flat roof windows are mostly inert and can be disposed
insignificant in terms of quantity.
of in an appropriate landfill. However, due to the value of the
materials or the carbon content of the plastic parts and wood,
The plastic packaging (polyethylene (PE) film, polystyrene foam
recycling or energy recovery is preferable and common.
parts) can be recycled if separated by type; alternatively, they
can be incinerated.
Waste code according to the European Waste List (Regulation
2.10 Condition of use on the European Waste List):
The material composition of VELUX flat roof windows does not
16 02 14 electronic parts
change over their service life.
17 02 01 wood
2.11 Environment and health during use 17 02 02 glass
VELUX flat roof windows do not contain any pollutants that 17 02 03 plastics
could be released during use. 17 04 14 mixed metals
2.16 Further information
Environmental protection: According to current knowledge,
Further documentation on the products, technical data sheets,
hazards to water, air and soil cannot arise when the products
BIM files, etc. can be found at:
are used as intended.
www.velux.com
3. LCA: Calculation rules
Name Value Unit
3.1 Declared Unit
Declared unit 1 pce.
The declared unit is 1 piece of a grid-connected VELUX flat
roof window CSF with a fixed base unit made of a PVC curb
Area 1.44 m2
with an integrated glazing unit with 1.20 m x 1.20 m = 1.44 m2. Weight 82,6 kg
Declared unit
3.2 System boundary
3 Environmental Product Declaration - VELUX A/S - VELUX flat roof window CVP - grid-connected
Type of EPD: Cradle to gate with options, with modules C1 – chapter 4.
C4, and module D (A1-A3, C1-C3, D and additional modules
3.4 Cut-off criteria
The production of VELUX flat roof windows (modules A1-A3) No data available from the company survey was neglected.
includes raw material extraction, energy generation, waste These include, among other things, material use, energy
treatment and all transports up to the factory gate. In demand (heat, electricity), packaging materials of raw materials
accordance with COUNCIL REGULATION (EU) No 333/2011, (insofar as they are generated as waste) and product
secondary metals are modeled as part of the product system packaging, consumables in production, waste treatment and
from the moment they are available as unmixed scrap. the transport of all inputs and outputs.
Waste or secondary fuels are not used for production. With this approach, mass and energy flows below 1 % were
also accounted for. No processes were neglected that would
Module A4 is not declared due to large variances in transport have been known to the project managers and would have
distances between the production site and the construction site, contributed significantly to the indicators of the impact
where the product is installed. assessment.
3.5 Background data
Module A5: The products are delivered to the construction site
ready to be installed. Manual installation is assumed, and Ecoinvent 3.8 (2021) is used as the background database.
electricity consumption related to electric drilling machines,
3.6 Data quality
screw drivers, etc. is considered to be negligible. The
The foreground data are based on extensive and detailed data
combustible packaging material (plastics, wood, etc.) is
collection at the production site. The foreground data could be
assumed to be thermally treated in a municipal waste
fully linked with corresponding data records from the
incineration plant with an efficiency R1 < 0.6 (according to the
background database ecoinvent 3.8.
ecoinvent dataset used); the recovered energy is declared as
The background data was updated in 2021. Thus, the quality of
exported energy. Metals and cardboard are recycled; it is
the foreground and background data can be rated as very
assumed that these fractions reach the end-of-waste state after
good.
having been sorted and transported (as a conservative choice)
to a recycler. No packaging waste is landfilled. 3.7 Period under review
The LCA data represents the production conditions for the year
Modules B1 to B7 are not relevant for the product under
2021.
consideration or no significant environmental impacts occur.
3.8 Geographic Representativeness
Module C1 includes manual dismantling, with no significant Land or region, in which the declared product system is
environmental impact. manufactured, used or handled at the end of the product´s
lifespan: Europe
Module C2 comprises the transport of the dismantled VELUX
flat roof window to a sorting plant and then to a waste
incineration plant for the thermally treated plastic fraction. 3.9 Allocation
No co-products are generated during the production of the
Modules C3/C4: given the complexity of the inventoried VELUX products. Sorted production scrap of the different
products, a mixed end-of-life scenario is modelled, allowing the metals, notably aluminium, is considered a secondary material
different materials to follow their most likely path. with no economic value (so no burdens allocated) and
As a rule of thumb, metals are recycled and plastics are considered in the quantification of net flows leaving the product
incinerated (also due to the very limited data availability of system. This approach is chosen to ensure a coherent
plastics recycling and its benefits); coated and uncoated flat quantification of net flows entering module D.
glass is assumed to be recycled whereas laminated glass is Biogenic carbon is allocated based on physical flows
assumed to be landfilled due to very limited recycling potential. regardless of the allocation procedure chosen for the process.
Metals and flat glass recycled; it is assumed that these fractions The biogenic carbon content of wood products entering or
reach an end-of-waste state after having been sorted and leaving the product system is quantified (manually) as part of
transported to a recycler; laminated glass is landfilled. The the GWP in conformity with DIN EN 16485.
combustible material (plastics, wood, etc.) is assumed to be
thermally treated in a municipal waste incineration plant. No processes were modelled as part of the foreground model
that would have required an allocation of multi-input processes.
Module D includes the benefits and burdens associated with Background datasets on municipal waste incineration plants
recycling metals beyond the system boundary, resulting from were taken from ecoinvent without any modification.
the treatment of recycled materials from the point of end-of-
waste to the point of substitution (as loads) and substitution of Allocation of reuse, recycling and recovery was avoided by the
primary resources (as benefits). cut-off approach in the foreground model in line with DIN EN
It also includes the benefits and burdens associated with 15804.
energy recovery from plastic waste in a municipal waste
incineration plant, as modeled in Module C3. 3.10 Comparability
In Module D, only net flows of metals leaving the product Basically, a comparison or an evaluation of EPD data is only
system are considered. possible if all the data sets to be compared were created
according to EN 15804 and the building context, respectively
3.3 Estimates and assumptions the product-specific characteristics of performance, are taken
No further assumptions and estimates relevant to the result had into account.
to be made beyond the points made in this chapter 3 and in
4. LCA: Scenarios and additional technical information
4 Environmental Product Declaration - VELUX A/S - VELUX flat roof window CVP - grid-connected
Name Value Unit
Characteristic product properties of biogenic carbon
Reference service life
according to
30 a
Information on describing the biogenic carbon content at manufacturer's
factury gate declaration
Name ValueUnit The product has passed
Declared product
kg internal quality controls and
Biogenic carbon content in product 0.097 properties (at the gate) -
C complies with EN 1873 for CE
and finishes
marking
Biogenic carbon content in accompanying kg
1.98
packaging C Design application
parameters (if instructed
Note: 1 kg of biogenic carbon is equivalent to 44/12 kg of CO .
2 by the manufacturer), Installation according to
including the references assembly instructions and -
to the appropriate state of the art.
practices and application
codes
An assumed quality of
Module A5
work, when installed in
The products are delivered to the construction site ready to be Carried out in accordance with
accordance with the -
installed. Manual installation is assumed; electricity the manufacturer's instructions.
manufacturer’s
consumption related to electric drilling machines, screw drivers,
instructions
etc. is considered to be negligible.
Outdoor environment, (for The declared products are
The combustible packaging material (plastics, wood, etc.) is
outdoor applications), e.g. intended for installation outside
assumed to be transported 50 km with a lorry 16-32 metric
weathering, pollutants, UVthe building: They are therefore
tons, EURO6 to an incineration plant with an efficiency R1 < 0.6 -
and wind exposure, designed to withstand outdoor
(according to the ecoinvent dataset used); the recovered
building orientation, conditions throughout their
energy is declared as exported energy; for its quantification an
shading, temperature service life.
efficiency of 25.6 % is assumed for the production of heat and
13.0 % for the production of electricity (always referring to the Indoor environment (for
The declared products are not
lower heating value of the waste). indoor applications), e.g.
intended for installation inside -
Metals and cardboard are recycled; it is assumed that these temperature, moisture,
a building.
fractions reach the end-of-waste state after having been sorted chemical exposure
and transported (as a conservative choice) to a recycler over Usage conditions, e.g. Standard use in any type of
150 km with a lorry 16-32 metric tons, EURO6. frequency of use, building, i.e. opening/closing -
No packaging waste is landfilled. mechanical exposure as often as necessary.
The use of multi-way pallets is not taken into account as The declared products are
packaging material. designed for a reference life of
Maintenance e.g. required
30 years, with the motor
frequency, type and
Reference service life replaced every 15 years. They -
quality and replacement
are maintained by cleaning
of components
water at the discretion of the
building occupants.
Module B1
The products are assumed to have no direct emissions during
the use phase. The indicator values of Module B1 are thus 0.
For biogenic carbon stored in product, see above.
Module B2
The maintenance scenario (B2) covers the replacement of the
motor over the service life of the product. Given that the
detailed composition of the motor and its electronic
components is not known, potential loads and benefits related
to the motor and electronics are disregarded.
Annual cleaning with water (e.g., using 1 l/m2 of tap water per
annual cleaning) is neglected.
Module B6
For motor-operated flat roof windows, electricity is used both in
stand-by and during operations.
Module C1
Manual de-installation is assumed, electricity consumption
related to electric screw drivers, etc. is considered to be
negligible. Thus, no environmental impacts are declared in
module C1.
Module C2
Given the complexity of the inventoried products, a mixed end-
5 Environmental Product Declaration - VELUX A/S - VELUX flat roof window CVP - grid-connected
of-life scenario is modelled, allowing the different materials to are recovered as heat and 13.0 % as electricity. Recovered
follow their most likely path. energy is reported as 'exported energy' and considered in
Module D.
It should also be noted that the deconstruction and waste
treatment scenario can vary a lot, depending on the actual Some of the material, notably laminated flat glass is assumed
situation. Thus, a generic end-of-life scenario is assumed. to be landfilled.
As a rule of thumb, metals are recycled, plastics are incinerated Module D
(also due to the very limited availability on plastics recycling Module D contains the benefits and loads beyond the system
and its benefits); coated and uncoated flat glass is assumed to boundary related to the recycling of metals, which result from
be recycled whereas laminated glass is assumed to be the treatment of recycled materials from the point of end-of-
landfilled due to very limited recycling potential. waste status to the point of substitution (as loads) and the
substitution of primary resources (as benefits).
The combustible material (plastics, wood, etc.) is assumed to
be transported 50 km with a lorry 16-32 metric tons, EURO6 to Furthermore, it includes the benefits of raw material substitution
an incineration plant. of the recycling of flat glass, with the exception of laminated
glass, which cannot be used for the production of glass again.
Metals and flat glass recycled; it is assumed that these fractions Recovered flat glass is assumed to have reached the end-of-
reach end-of-waste state after having been sorted and waste state as sorted glass cullet; glass cullet is assumed to
transported to a recycler over 150 km with a lorry 16-32 metric replace virgin raw material for glass production – impacts on
tons, EURO6. the energy required to remelt recycled glass as compared to
virgin glass production are neglected due to a lack of data.
Laminated glass is landfilled, including a transport of 30 km with
a lorry 16-32 metric tons, EURO6. It also includes the benefits and loads related to the energy
recovery from plastic wastes in a MWIP as modelled in
Module C3 Modules A3, A5 and C3.
A consumption of 0.03 kWh/kg of electricity for shredding and
sorting and 0.437 MJ/kg of diesel fuel for internal logistics are The benefits of the recycling of the motor and electronic parts
taken into account to disassemble the product. The recovered are not considered due to the absence of data on its
material leaves the product system as 'materials for recycling'. composition and recycled content.
The net amounts of the metals leaving the product system are
considered as 'use of secondary material' in Module D. Due to a lack of data for plastics from de-construction activities,
the substitution potential of recycled plastics is not taken into
Module C4 account.
As stated above, it is assumed that 100 % of the plastic parts
and the wooden parts are treated in a waste incineration plant Only net flows leaving the product system are considered in
with an efficiency R1 < 0.6 (according to the ecoinvent dataset module D.
used); 25.57 % of the lower heating value of the plastic parts
6 Environmental Product Declaration - VELUX A/S - VELUX flat roof window CVP - grid-connected
5. LCA: Results
Disclaimer:
EP-freshwater: This indicator has been calculated as 'kg P eq' as required in the characterization model (EUTREND model, Struijs et
al., 2009b, as implemented in ReCiPe; http://eplca.jrc.ec.europa.eu/LCDN/developerEF.xhtml)
DESCRIPTION OF THE SYSTEM BOUNDARY (X = INCLUDED IN LCA; MND = MODULE OR INDICATOR NOT DECLARED; MNR
= MODULE NOT RELEVANT)
Benefits and
Construction loads beyond
Product stage Use stage End of life stage
process stage the system
boundaries
la ire ta m w a Ry lp p u s tro p s n a rT g n iru tc a fu n a M e h t m o rf tro p s n a rTe tis e h t o t e ta g y lb m e s s A e s U e c n a n e tn ia M ria p e R tn e m e c a lp e R tn e m h s ib ru fe R y g re n e la n o ita re p Oe s u re ta w la n o ita re p Oe s u n o itc u rts n o c -e Dn o itilo m e d tro p s n a rT g n is s e c o rp e ts a W la s o p s iD -e s u e R-y re v o c e R-g n ilc y c e Rla itn e to p
A1 A2 A3 A4 A5 B1 B2 B3 B4 B5 B6 B7 C1 C2 C3 C4 D
X X X MND X X X MNR MNR MNR X MND X X X X X
RESULTS OF THE LCA - ENVIRONMENTAL IMPACT according to EN 15804+A2: 1 piece VELUX flat roof window CVP - grid-
connected, 1.20 m x 1.20 m = 1.44 m2
Parameter Unit A1-A3 A5 B1 B2 B6 C1 C2 C3 C4 D
GWP-total kg CO 2 eq 2.44E+02 9.23E+00 0 5.83E+01 1.36E+02 0 6.11E-01 2.97E+00 1.38E+02 -4.56E+01
GWP-fossil kg CO 2 eq 2.51E+02 1.95E+00 0 5.83E+01 1.36E+02 0 6.11E-01 2.61E+00 1.38E+02 -4.56E+01
GWP-
biogenic kg CO 2 eq -7.63E+00 7.27E+00 0 0 0 0 0 3.6E-01 0 0
GWP-luluc kg CO 2 eq 2.19E-01 8.66E-05 0 2E-02 3.39E-01 0 2.49E-04 1.96E-03 3.53E-02 -5.41E-02
ODP kg CFC11 eq 5.69E-05 4.9E-08 0 2.04E-06 6.88E-06 0 1.43E-07 1.1E-07 1.18E-05 -3.16E-06
AP mol H+ eq 1.21E+00 1.35E-03 0 2.21E-01 6.99E-01 0 3.46E-03 6.92E-03 1.5E-01 -1.24E-01
EP-
kg P eq 8.32E-03 1.65E-06 0 1.52E-03 1.53E-02 0 4.49E-06 2.25E-04 1.03E-03 -3.37E-03
freshwater
EP-marine kg N eq 2.12E-01 5.05E-04 0 1.13E-01 8.96E-02 0 1.24E-03 2.25E-03 1.22E-01 -2.18E-02
EP-terrestrial mol N eq 2.29E+00 5.59E-03 0 3.33E-01 1.04E+00 0 1.37E-02 2.54E-02 4.07E-01 -2.53E-01
kg NMVOC
POCP 7.38E-01 1.58E-03 0 1.09E-01 2.83E-01 0 3.92E-03 6.75E-03 1.2E-01 -7.86E-02
eq
ADPE kg Sb eq 5.38E+02 7.18E-07 0 4.3E-03 3.29E-04 0 2.05E-06 3.11E-06 2.62E-04 -1.24E-04
ADPF MJ 3.48E+03 3.21E+00 0 2.38E+02 2.88E+03 0 9.4E+00 2.43E+01 3.23E+02 -6.22E+02
m3 world eq
WDP 9.78E+01 1.31E-02 0 9.36E+00 3.21E+01 0 3.09E-02 1.11E-01 2.13E+01 -2.88E+00
deprived
GWP = Global warming potential; ODP = Depletion potential of the stratospheric ozone layer; AP = Acidification potential of land and water; EP =
Eutrophication potential; POCP = Formation potential of tropospheric ozone photochemical oxidants; ADPE = Abiotic depletion potential for non-fossil
resources; ADPF = Abiotic depletion potential for fossil resources; WDP = Water (user) deprivation potential)
RESULTS OF THE LCA - INDICATORS TO DESCRIBE RESOURCE USE according to EN 15804+A2: 1 piece VELUX flat roof
window CVP - grid-connected, 1.20 m x 1.20 m = 1.44 m2
Parameter Unit A1-A3 A5 B1 B2 B6 C1 C2 C3 C4 D
PERE MJ 1.81E+02 4.87E-02 0 2.21E+01 5.46E+02 0 1.33E-01 3.05E+00 2.85E+01 -5.68E+01
PERM MJ 8.82E+01 -8.35E+01 0 0 0 0 0 -4.64E+00 0 0
PERT MJ 2.69E+02 -8.35E+01 0 2.21E+01 5.46E+02 0 1.33E-01 -1.59E+00 2.85E+01 -5.68E+01
PENRE MJ 3.27E+03 2.96E+01 0 2.37E+02 2.9E+03 0 9.4E+00 2.02E-05 1.19E+03 -6.29E+02
PENRM MJ 8.92E+02 -2.64E+01 0 0 0 0 0 0 -8.65E+02 0
PENRT MJ 4.16E+03 3.21E+00 0 2.37E+02 2.9E+03 0 9.4E+00 2.02E-05 3.24E+02 -6.29E+02
SM kg 1.78E+01 0 0 1.03E+00 0 0 0 0 0 -6.65E+00
RSF MJ 0 0 0 0 0 0 0 0 0 0
NRSF MJ 0 0 0 0 0 0 0 0 0 0
FW m3 2.27E+00 6.44E-04 0 1.46E-01 1.85E+00 0 1.02E-03 6.46E-03 4.75E-01 -1.44E-01
PERE = Use of renewable primary energy excluding renewable primary energy resources used as raw materials; PERM = Use of renewable primary
energy resources used as raw materials; PERT = Total use of renewable primary energy resources; PENRE = Use of non-renewable primary energy
excluding non-renewable primary energy resources used as raw materials; PENRM = Use of non-renewable primary energy resources used as raw
materials; PENRT = Total use of non-renewable primary energy resources; SM = Use of secondary material; RSF = Use of renewable secondary fuels;
NRSF = Use of non-renewable secondary fuels; FW = Use of net fresh water
RESULTS OF THE LCA – WASTE CATEGORIES AND OUTPUT FLOWS according to EN 15804+A2:
1 piece VELUX flat roof window CVP - grid-connected, 1.20 m x 1.20 m = 1.44 m2
Parameter Unit A1-A3 A5 B1 B2 B6 C1 C2 C3 C4 D
HWD kg 2.08E-02 8.48E-06 0 4.22E-03 1.02E-03 0 2.4E-05 2.02E-05 5.42E-04 2.35E-04
NHWD kg 5.4E+01 2.31E-01 0 3.41E+02 1.08E+01 0 6.3E-01 5.23E-01 3.72E+02 -8.23E+00
7 Environmental Product Declaration - VELUX A/S - VELUX flat roof window CVP - grid-connected
RWD kg 2.01E-02 4.57E-05 0 1.83E-03 3.87E-02 0 1.36E-04 2.19E-04 2.88E-03 -2.54E-03
CRU kg 0 0 0 0 0 0 0 0 0 0
MFR kg 8.97E+00 4.98E+00 0 2.16E+00 0 0 0 1.15E+01 0 0
MER kg 0 0 0 0 0 0 0 0 0 0
EEE MJ 1.12E+00 3.43E+00 0 1.21E-01 0 0 0 0 1.13E+02 0
EET MJ 2.11E+00 6.75E+00 0 2.38E-01 0 0 0 0 2.21E+02 0
HWD = Hazardous waste disposed; NHWD = Non-hazardous waste disposed; RWD = Radioactive waste disposed; CRU = Components for re-use;
MFR = Materials for recycling; MER = Materials for energy recovery; EEE = Exported electrical energy; EET = Exported thermal energy
RESULTS OF THE LCA – additional impact categories according to EN 15804+A2-optional:
1 piece VELUX flat roof window CVP - grid-connected, 1.20 m x 1.20 m = 1.44 m2
Parameter Unit A1-A3 A5 B1 B2 B6 C1 C2 C3 C4 D
Disease
PM 9.2E-06 1.98E-08 0 1.52E-06 1.79E-06 0 5.49E-08 1.04E-07 1.5E-06 -1.07E-06
incidence
IR kBq U235 eq 6.32E+00 1.38E-02 0 8.14E-01 2.62E+01 0 4.08E-02 8.44E-02 1.37E+00 -1.05E+00
ETP-fw CTUe 6.17E+03 3.74E+00 0 1.97E+03 1.45E+03 0 7.45E+00 1.94E+01 4.88E+03 -4.9E+02
HTP-c CTUh 4.87E-07 3.16E-10 0 1.05E-07 3.87E-08 0 2.97E-10 4.54E-10 3.34E-08 -5.64E-08
HTP-nc CTUh 5.6E-06 4.53E-09 0 2.08E-06 1.26E-06 0 8.57E-09 2.4E-08 1.27E-06 6.55E-08
SQP SQP 9.26E+02 2.7E+00 0 2.89E+02 4.42E+02 0 8.02E+00 3.46E+00 2.76E+02 -7.06E+01
PM = Potential incidence of disease due to PM emissions; IR = Potential Human exposure efficiency relative to U235; ETP-fw = Potential comparative
Toxic Unit for ecosystems; HTP-c = Potential comparative Toxic Unit for humans (cancerogenic); HTP-nc = Potential comparative Toxic Unit for humans
(not cancerogenic); SQP = Potential soil quality index
Disclaimer 1 – for the indicator 'Potential Human exposure efficiency relative to U235'.This impact category deals mainly with the
eventual impact of low dose ionizing radiation on human health of the nuclear fuel cycle. It does not consider effects due to possible
nuclear accidents, occupational exposure or radioactive waste disposal in underground facilities. Potential ionizing radiation from the
soil, radon and from some construction materials is also not measured by this indicator.
Disclaimer 2 – for the indicators 'abiotic depletion potential for non-fossil resources', 'abiotic depletion potential for fossil resources',
'water (user) deprivation potential, deprivation-weighted water consumption', 'potential comparative toxic unit for ecosystems', 'potential
comparative toxic unit for humans – cancerogenic', 'Potential comparative toxic unit for humans - not cancerogenic', 'potential soil
quality index'. The results of this environmental impact indicator shall be used with care as the uncertainties on these results are high
as there is limited experience with the indicator.
6. LCA: Interpretation
Figure 1 illustrates the relative contributions of the different
modules along the life cycle of the declared products.
one impact category to another.
Benefits and burdens beyond the system boundary (module D)
Figure 1: Relative environmental impacts of the different are in the order of 0 % to 15% of the impacts over the product
life cycle stages for the flat roof window CVP mains life cycle (modules A1-C4). [1] The use of renewable primary
energy is mainly caused by the share of renewable energy in
The largest part of environmental impacts is caused during the electricity mix, thus the production stage is the main drivers
production (modules A1-A3) ranging from 31% to roughly of this impact category; for the use of non-renewable primary
100%, and during the generation of operational energy (module energy, the operational energy (module B6) is the most
B2) The relative contributions of these main drivers differs from impacting life cycle stage.
8 Environmental Product Declaration - VELUX A/S - VELUX flat roof window CVP - grid-connected
Material use of primary energy is negligible and related to during disposal of the product; hazardous and radio-active
plastic parts of the product and packaging material. The wastes are mainly caused by the European electricity mix
material use of primary energy is transferred to its energy use
when the materials containing primary energy are incinerated [1] Benefits resulting from the recycling of plastics as well as
with energy recovery. from the recycling of the electronic parts are disregarded due to
the lack of data on the recycling processes and related to the
Non-hazardous waste as the quantitatively most relevant waste detailed composition of the electronic parts.
flows is mainly caused during the production of the glass and
7. Requisite evidence
to AltholzVO
8.1 Formaldehyde Not applicable; not tested based on applicable product
Not tested based on applicable product standard. standard. 7.4. Fire gas toxicity
Not tested based on applicable product standard. 7.5 VOC
7.2 MDI emissions
Not tested based on applicable product standard. 7.3 Not tested based on applicable product standard.
Checking of pre-treatment of substances used according
8. References
Product category rules of IBU methods.
IBU (2021) EN 12101-2
IBU (2021): General Instructions for the EPD Programme of the DIN EN 12101-2:2017-08, Smoke and heat control systems –
Institut Bauen & Umwelt e.V. (General Instructions for the IBU Part 2: Specification for natural smoke and heat exhaust
EPD Programme). Version 2.0, Institut Bauen & Umwelt, Berlin ventilators.
IBU (2017) EN 16485
IBU (2017): PCR Teil A: PCR Part A: Calculation rules for the DIN EN 16485:2014-07, Round and sawn timber -
life cycle assessment and requirements for the project report. Environmental Product Declarations - Product category rules
Version 1.8., Institut Bauen & Umwelt, Berlin. for wood and wood-based products for use in construction;
German version EN 16485:2014.
IBU (2021)
IBU (2021):PCR Part B: Requirements on the EPD for windows ECHA-List
and doors. Version 2021/01, Institut Bauen & Umwelt, Berlin. The Candidate List of substances of very high concern,
available via https://echa.europa.eu/nl/-/four-newsubstances-
Standards and legal documents added-to-the-candidate-list.
EN 15804 Regulation on biocidal products
DIN EN 15804+A2:2019, Sustainability of construction works - REGULATION (EU) No 528/2012 OF THE EUROPEAN
Environmental product declarations - Core rules for the product PARLIAMENT AND OF THE COUNCIL of 22 May 2012
category construction products. concerning the making available on the market and use of
biocidal products.
ISO 14025
DIN EN ISO 14025:2006-07, Environmental labels and Regulation (EU) Nr. 305/2011(CPR)
declarations - Type III Environmental declarations - Principles REGULATION (EU) No 305/2011 OF THE EUROPEAN
and procedures. PARLIAMENT AND OF THE COUNCIL of 9 March 2011 laying
down harmonised conditions for the marketing of construction
ISO 14044 products and repealing Council Directive 89/106/EEC.
DIN EN ISO 14044:2006-07, Environmental management - Life
cycle assessment - Requirements and guidance (ISO COUNCIL REGULATION (EU) No 333/2011
14044:2006); German and English versions EN ISO COUNCIL REGULATION (EU) No 333/2011 of 31 March 2011
14044:2006. establishing criteria determining when certain types of scrap
metal cease to be waste under Directive 2008/98/EC of the
ISO 9001 European Parliament and of the Council.
DIN EN ISO 9001:2015, Quality management systems -
Requirements. European Waste List (Waste index)
http://www.gesetze-im-internet.de/avv/anlage.htm
ISO 14001
DIN EN ISO 14001:2015: Environmental management Additional references
systems - Requirements with guidance for use.
Weidema et al. (2013)
ISO 45001 Weidema, B., C. Bauer, R. Hischier, C. Mutel, T. Nemecek, J.
ISO 45001:2018-03, Occupational health and safety Reinhard, C.O. Vadenbo, G. Wernet (2013): Overview and
management systems - Requirements with guidance for use. methodology, Data quality guideline for the ecoinvent database
version 3. ecoinvent report no. 1 (v3), St. Gallen, Schweiz.
EN 1873
DIN EN 1873:2005, Prefabricated accessories for roofing - ecoinvent 3.8
Individual rooflights of plastics - Product specification and test ecoinvent 3.8, LCA database, 12/2021. Ecoinvent centre,
9 Environmental Product Declaration - VELUX A/S - VELUX flat roof window CVP - grid-connected
Zürich.
10 Environmental Product Declaration - VELUX A/S - VELUX flat roof window CVP - grid-connected
Publisher
Institut Bauen und Umwelt e.V. +49 (0)30 3087748- 0
Hegelplatz 1 info@ibu-epd.com
10117 Berlin www.ibu-epd.com
Germany
Programme holder
Institut Bauen und Umwelt e.V. +49 (0)30 3087748- 0
Hegelplatz 1 info@ibu-epd.com
10117 Berlin www.ibu-epd.com
Germany
Author of the Life Cycle Assessment
Dr. Frank Werner - Umwelt & Entwicklung + 41 (0)44 241 39 06
Kammelenbergstrasse 30 frank@frankwerner.ch
9011 St. Gallen http://www.frankwerner.ch/
Switzerland
Owner of the Declaration
VELUX Group +4545164726
Ådalsvej 99 jakob.roerbech@velux.com
2970 Hørsholm www.velux.com
Denmark
11 Environmental Product Declaration - VELUX A/S - VELUX flat roof window CVP - grid-connected
