ENVIRONMENTAL PRODUCT DECLARATION
as per ISO 14025 and EN 15804+A2
Owner of the Declaration Lanxess Deutschland GmbH, BU Inorganic Pigments
Publisher Institut Bauen und Umwelt e.V. (IBU)
Programme holder Institut Bauen und Umwelt e.V. (IBU)
Declaration number EPD-LAN-20230193-IBC2-EN
Issue date 10.08.2023
Valid to 09.08.2028
Iron Hydroxide Yellow Pigment (FeOOH)
Lanxess Deutschland GmbH
www.ibu-epd.com | https://epd-online.com
1. General Information
Lanxess Deutschland GmbH Iron Hydroxide Yellow Pigment (FeOOH)
Programme holder Owner of the declaration
IBU – Institut Bauen und Umwelt e.V. Lanxess Deutschland GmbH, BU Inorganic Pigments
Hegelplatz 1 Rheinuferstr. 7 - 9
10117 Berlin 47829 Krefeld
Germany Germany
Declaration number Declared product / declared unit
EPD-LAN-20230193-IBC2-EN 1,000 kg iron hydroxide yellow pigment
(weighted average)
This declaration is based on the product category rules: Scope:
Inorganic Pigments in Various Forms of Delivery, 01.08.2021 This EPD applies to iron hydroxide yellow pigments in the versions
(PCR checked and approved by the SVR) compacted, powder, granulate and micronized (different versions for each
of the brand names). It is an average EPD for which the weighted average
of the five versions was calculated on the basis of the mass-specific
Issue date production rate of the year 2021. Production of the pigments from one
factory in Germany was assessed.
10.08.2023
The owner of the declaration shall be liable for the underlying information
and evidence; the IBU shall not be liable with respect to manufacturer
Valid to
information, life cycle assessment data and evidences.
09.08.2028
The EPD was created according to the specifications of EN 15804+A2. In
the following, the standard will be simplified as EN 15804.
Verification
The standard EN 15804 serves as the core PCR
Independent verification of the declaration and data according to ISO
14025:2011
internally X externally
Dipl.-Ing. Hans Peters
(Chairman of Institut Bauen und Umwelt e.V.)
Florian Pronold Matthias Klingler,
(Managing Director Institut Bauen und Umwelt e.V.) (Independent verifier)
1 Environmental Product Declaration - Lanxess Deutschland GmbH - Iron Hydroxide Yellow Pigment (FeOOH)
2. Product
additives used must comply with EN 934-1, annex A.1.
2.1 Product description/Product definition
Inorganic pigments are defined as substances that are The extremal values (worst-case assessment) across the three
insoluble in the application medium (ISO 18451-1) and assessed versions are used to prove conformity with the
manufactured by means of chemical synthesis. This EPD standard.
covers the product iron hydroxide yellow pigment in its typical
versions, namely powder, granulate, compacted and Performance figures for the product in line with the declaration
micronized. of performance in relation to its key characteristics as per DIN
EN 12878:2014 Pigments for the colouring of building materials
The average values of the inorganic pigments declared here based on cement and/or lime - Specifications and methods of
are based on the product volume in the indicated versions. test.
Regulation (EU) no. 305/2011 (CPR) applies to the placing of 2.4 Delivery status
the product on the market in the EU/EFTA (except Switzerland). Typical versions of the iron hydroxide yellow pigment are
The product requires a declaration of performance with due powder, compacted, granulate and micronized. The packaging
consideration of DIN EN 12878:2014 Pigments for the colouring typically ranges from 25 kg polyethylene (PE) / paper sacks to
of building materials based on cement and/or lime - big bags with a net weight of one metric ton. The calculations in
Specifications and methods of test, and CE marking. The this EPD are based on an assessment of big-bag material. As
respective national provisions apply to use. the packaging material accounts for a very small proportion of
the calculated environmental impacts, only big bags made from
2.2 Application polypropylene (PP) and low-density polyethylene (LDPE) were
Inorganic iron oxide pigments are used for colouring building assessed as the packaging material.
materials made from cement, cement/lime mixtures, lime
mortar, and bituminous applications. Other applications include 2.5 Base materials/Ancillary materials
use in paints and coatings as well as plastics. On average, iron hydroxide yellow pigment is made up of the
following raw and auxiliary materials:
2.3 Technical Data
Name Value Unit
The product technical data that comes within the scope of the
Sodium hydroxide 58,0 %
EPD is set out in the table below, with reference to the check
rules based on EN 12878. Ferrous sulfate 31,6 %
Aluminum sulfate 3,2 %
Structural data - Influence on cement properties Sodium aluminate 2,2 %
Name Value Unit Iron pellets (93%) 1,5 %
Setting time (start of setting process min. 1h) 160 min Iron (II) chloride 1,4 %
Setting time (end of setting time max. 12h) 260 min Phosphoric acid 0,3 %
Influence on cement setting (delta mixture with Iron scrap 0,2 %
-47 min
and without pigment max. + 60 min.) Aluminum chloride 0,1 %
Compressive strength (mortar 28 days (compare Cooling water 1,6 %
-0.8 N/mm2
mixture with and without pigment)) (category A)
1) The product/at least one partial product contains substances
Compressive strength (mortar 28 days (compare on the ECHA list of substances of very high concern (SVHC)
mixture with and without pigment)) (category B, -1.9 N/mm2 (date July 8, 2021) above 0.1 % by mass: No.
max. -8%)
Chloride content (total chloride; category A) 0.14 % 2) The product/at least one partial product contains further
Chloride content (total chloride; category B, max. carcinogenic, mutagenic, reprotoxic (CMR) substances in
0.03 %
0.1%) category 1A or 1B that are not on the candidate list, above 0.1
% by mass in at least one partial product: No.
Soluble chloride content (category A) 0.07 %
Soluble chloride content (total chloride; category
0.03 % 3) This construction product has had biocidal products added to
B, max. 0.1%)
it, or it has been treated with biocidal products (it is therefore a
Content of water-soluble substances (category 1.14 % treated article as per the Biocidal Products Regulation (EU) no.
A) 528/2012): No
Content of water-soluble substances (category
B, max. 0.5%) 1.29 % 2.6 Manufacture
A solution of iron sulfate that is designated as waste product
*) Provided that the water-soluble content complies with EN
from the steel industry is mixed with sodium hydroxide in a
934-1.
controlled manner with the addition of air or oxygen.
The amount of water-soluble substances as defined by EN 934-
2 FeSO + 4 NaOH +½ O → 2 FeOOH + 2 Na SO + H O
1, paragraph 5.2.3, must not exceed: 4 2 2 4 2
• Category A: the level stated by the manufacturer
After subsequent drying, washing is carried out, followed by
• Category B: 0.5 % by mass for individual pigments and
grinding.
pigment mixtures. If additives such as dispersants,
binders, and/or grinding aids are used for powder or
non-powder preparations, their water-soluble total 2.7 Environment and health during manufacturing
content must be equal to or less than 5.5 % by mass
(8.0 % for carbon black) in relation to the solid. The
2 Environmental Product Declaration - Lanxess Deutschland GmbH - Iron Hydroxide Yellow Pigment (FeOOH)
LANXESS is continuously investing in modern manufacturing The product is not a hazardous substance (as per the CLP
processes at all locations. The Inorganic Pigments business Regulation). There is no risk if the product is handled and
unit and its equipment are certified according to ISO 9001, processed in compliance with the applicable regulations in the
14001, and 50001. workplace.
Iron oxide pigments are certified by SCS Global Services for 2.12 Reference service life
their high content of recycled raw materials. This EPD assesses modules A1–A3 (cradle to gate). The
service life corresponds to typical use in the respective
2.8 Product processing/Installation application
As this EPD assesses modules A1–A3 (cradle to gate); a rough
description of the application processes is attached. 2.13 Extraordinary effects
Fire
Customers typically use dosing units to dose iron oxide FeOOH is non-flammable.
pigments into specific color mixtures and to process them into
cement-bound, lime-bound, orbituminous products. Water
No hazardous substances are released as a result of contact
2.9 Packaging with water.
All versions of the pigments are packaged identically. The
finished product is usually packaged in PE/paper sacks with a Mechanical destruction
net weight of 25 kg through to big bags made of PP and LDPE Not applicable.
with a net weight of one metric ton.
2.14 Re-use phase
According to the German Association for Plastics Packaging This EPD assesses modules A1–A3 (cradle to gate). As iron
and Films (IK), the big bags made of PP and LDPE on which hydroxide yellow pigments are bound in the application
the calculations of the EPD are based can be reused in a medium, reuse is not pursued on account of the substantial
closed-loop system under specific conditions for the same amount of thermal energy required and the technical options
product (max. 2 years). The big bags can be recycled at the currently available. Recycling management provides individual
end of their life. For mechanical recycling, the used synthetic opportunities for the use of the bound pigment.
fabrics are treated mechanically with no change to the chemical
structure. The recycled materials can be used in various 2.15 Disposal
applications and replace new granulate. Disposal is carried out in conjunction with and in accordance
with the respective application medium.
2.10 Condition of use The waste code for iron oxide is 060316 (as per the German
This EPD assesses modules A1–A3 (cradle to gate). No Waste Catalog Ordinance).
material changes are expected within the recommended usage
limits. 2.16 Further information
Further information on iron hydroxide yellow pigments and
further Lanxess IPG products and services is available at
www.bayferrox.com
2.11 Environment and health during use
3. LCA: Calculation rules
A1: Supply of raw materials
3.1 Declared Unit A2: Transportation of raw materials to the manufacturer
The selected declared unit relates to an average product. The A3: Manufacture of the product (including required energy and
average was formed as a weighted mean from the annual water) and manufacture of the product packaging
production quantities of the compacted, powder, granulate and
micronized versions in the year 2021 (reference to mass). 3.3 Estimates and assumptions
Primary data across all versions were used for transportation of
Declared unit and mass reference
the iron filings (module A2) and for on-site production
Name Value Unit
processes at Lanxess Deutschland GmbH (module A3). A
Declared unit 1000 kg distance of 1,000 km (within Europe) was assumed for
transportation of all further input materials (module A2).
Electricity consumption of 0.072 MJ per t km was assumed for
3.2 System boundary transportation via pipeline.
Type of EPD: Cradle to gate with options
Only modules A1 to A3 were calculated because the pigment Generic data was used for the production of raw materials
fulfills all of the below criteria, as stated in PCR Part A: (module A1) as these are not produced by Lanxess
Deutschland GmbH itself and no detailed information was
• the product is physically integrated with other products
available.
during installation so they cannot be physically
separated from them at the end of life,
Credits for the avoidance of generation of electricity and steam
• the product is no longer identifiable at the end of life as
in another product system through the incineration processes
a result of a physical or chemical transformation
for production waste were also taken into account. 100 %
process,
incineration including energy recovery in the closed-loop
• the product does not contain biogenic carbon.
method to A3 (electricity and steam) was assumed here.
The following modules were taken into account in the LCA 3.4 Cut-off criteria
calculation
3 Environmental Product Declaration - Lanxess Deutschland GmbH - Iron Hydroxide Yellow Pigment (FeOOH)
All primary data of the production processes were taken into in this period and then correspondingly subjected to average
account. No cut-off rules were applied. weighting for the average assessment.
3.5 Background data 3.8 Geographic Representativeness
The software system GaBi 10 developed by Sphera was used Land or region, in which the declared product system is
for modelling the product's LCA. The data sets contained manufactured, used or handled at the end of the product´s
therein are either from the GaBi Professional database (v lifespan: Germany
2023.1) or from the Ecoinvent database (v 3.8).
3.6 Data quality 3.9 Allocation
The GaBi software system for life-cycle analyses and the GaBi Module A1 does not take account of any debits for the iron
Professional database (v 2023.1), as well as the Ecoinvent sulfate used as this is pre-consumer material as per ISO 14021.
database (v 3.8) were used for life-cycle modeling of the Some of the material used stems from ilmenite treatment at a
assessed products. The produced quantities for 2022 were titanium dioxide factory, and some of it stems from pig-iron
gathered by Lanxess. pickling plants in the steel industry.
Corresponding data sets were available for the input materials All credits from recovered energy from processes relating to the
used, and some of them have been adapted with regard to incineration of production waste were allocated to A3 with the
concentration. The age of the background data used (2018– closed-loop method.
2021) is less than 15 years and can be regarded as
3.10 Comparability
representative for the assessment period.
Basically, a comparison or an evaluation of EPD data is only
The LCA figures for the average EPD (weighted mean for the possible if all the data sets to be compared were created
year 2021) can be regarded as robust as they are a weighted according to EN 15804 and the building context, respectively
average of high-quality, measured activity data. All data used the product-specific characteristics of performance, are taken
can be regarded as representative. into account. Background data was taken from the GaBi
Professional database (v 2023.1). To fill occasional gaps,
3.7 Period under review datasets from the Ecoinvent database (v 3.8) were used.
The assessment period is 2021. All in-house data was gathered
4. LCA: Scenarios and additional technical information
in the context of a building assessment if modules are not
Characteristic product properties of biogenic carbon declared (MND).
The content of biogenic carbon in the product is 0 %. The
product packaging consists of plastic (PP) without biogenic As disposal of the packaging material on the buildingsite
content. (module A5) is not declared, the assessed quantities of
packaging materials are stated below:
• Big bag (PP): 2.05 kg/1,000 kg product
Technical Information
• Big bag (LDPE): 0.72 kg/1,000 kg product
The following technical information forms the basis for the
declared modules or can be used to develop specific scenarios
4 Environmental Product Declaration - Lanxess Deutschland GmbH - Iron Hydroxide Yellow Pigment (FeOOH)
5. LCA: Results
The following tables show the environment-relevant results as per EN 15804 for 1,000 kg iron hydroxide yellow pigment (weighted
average for the compacted, powder, granulate and two micronized versions).
DESCRIPTION OF THE SYSTEM BOUNDARY (X = INCLUDED IN LCA; ND = MODULE OR INDICATOR NOT DECLARED; MNR =
MODULE NOT RELEVANT)
Benefits and
Construction loads beyond
Product stage Use stage End of life stage
process stage the system
boundaries
la ire ta m w a Ry lp p u s tro p s n a rT g n iru tc a fu n a M e h t m o rf tro p s n a rTe tis e h t o t e ta g y lb m e s s A e s U e c n a n e tn ia M ria p e R tn e m e c a lp e R tn e m h s ib ru fe R y g re n e la n o ita re p Oe s u re ta w la n o ita re p Oe s u n o itc u rts n o c -e Dn o itilo m e d tro p s n a rT g n is s e c o rp e ts a W la s o p s iD -e s u e R-y re v o c e R-g n ilc y c e Rla itn e to p
A1 A2 A3 A4 A5 B1 B2 B3 B4 B5 B6 B7 C1 C2 C3 C4 D
X X X MND MND MND MND MNR MNR MNR MND MND MND MND MND MND MND
RESULTS OF THE LCA - ENVIRONMENTAL IMPACT according to EN 15804+A2: 1000 kg Iron Hydroxide Yellow Pigment
Parameter Unit A1-A3 A1 A2 A3
Global Warming Potential total (GWP-total) kg CO 2 eq 2.22E+03 1.05E+03 1.54E+02 1.01E+03
Global Warming Potential fossil fuels (GWP-fossil) kg CO 2 eq 2.19E+03 1.04E+03 1.54E+02 9.94E+02
Global Warming Potential biogenic (GWP-biogenic) kg CO 2 eq 2.91E+01 9.19E+00 -5.7E-01 2.05E+01
Global Warming Potential luluc (GWP-luluc) kg CO 2 eq 1.22E+00 5.88E-01 5.85E-01 4.88E-02
Depletion potential of the stratospheric ozone layer (ODP) kg CFC11 eq 5.18E-06 5.18E-06 7.88E-11 9.82E-10
Acidification potential of land and water (AP) mol H+ eq 4.08E+00 2.88E+00 4.12E-01 7.82E-01
Eutrophication potential aquatic freshwater (EP-freshwater) kg P eq 3.76E-02 3.71E-02 3.12E-04 1.71E-04
Eutrophication potential aquatic marine (EP-marine) kg N eq 1.17E+00 6.73E-01 1.86E-01 3.07E-01
Eutrophication potential terrestrial (EP-terrestrial) mol N eq 1.31E+01 7.66E+00 2.08E+00 3.37E+00
kg NMVOC
Formation potential of tropospheric ozone photochemical oxidants (POCP) 2.99E+00 1.75E+00 3.77E-01 8.59E-01
eq
Abiotic depletion potential for non fossil resources (ADPE) kg Sb eq 2.26E-03 2.19E-03 1.62E-05 5.73E-05
Abiotic depletion potential for fossil resources (ADPF) MJ 3.28E+04 1.5E+04 2.04E+03 1.57E+04
m3 world eq
Water use (WDP) 8.22E+01 6.87E+01 7E-01 1.29E+01
deprived
RESULTS OF THE LCA - INDICATORS TO DESCRIBE RESOURCE USE according to EN 15804+A2: 1000 kg Iron Hydroxide
Yellow Pigment
Parameter Unit A1-A3 A1 A2 A3
Renewable primary energy as energy carrier (PERE) MJ 7.06E+03 6.56E+03 1.54E+02 3.42E+02
Renewable primary energy resources as material utilization (PERM) MJ 0 0 0 0
Total use of renewable primary energy resources (PERT) MJ 7.06E+03 6.56E+03 1.54E+02 3.42E+02
Non renewable primary energy as energy carrier (PENRE) MJ 3.28E+04 1.51E+04 2.04E+03 1.57E+04
Non renewable primary energy as material utilization (PENRM) MJ 1.26E+02 0 0 1.26E+02
Total use of non renewable primary energy resources (PENRT) MJ 3.29E+04 1.51E+04 2.04E+03 1.58E+04
Use of secondary material (SM) kg 2.26E+03 2.26E+03 1.41E-02 2.72E-01
Use of renewable secondary fuels (RSF) MJ 0 0 0 0
Use of non renewable secondary fuels (NRSF) MJ 0 3.27E-07 1.59E-09 6.16E-07
Use of net fresh water (FW) m3 1.29E+01 8.52E+00 1.17E+00 3.16E+00
RESULTS OF THE LCA – WASTE CATEGORIES AND OUTPUT FLOWS according to EN 15804+A2:
1000 kg Iron Hydroxide Yellow Pigment
Parameter Unit A1-A3 A1 A2 A3
Hazardous waste disposed (HWD) kg 4.43E-06 1.66E-06 1.17E-08 2.76E-06
Non hazardous waste disposed (NHWD) kg 3.69E+01 3E+01 3.54E-01 6.48E+00
Radioactive waste disposed (RWD) kg 1.19E+00 7.27E-01 4.87E-03 4.54E-01
Components for re-use (CRU) kg 0 0 0 0
Materials for recycling (MFR) kg 0 0 0 0
Materials for energy recovery (MER) kg 0 0 0 0
Exported electrical energy (EEE) MJ 0 0 0 0
Exported thermal energy (EET) MJ 0 0 0 0
RESULTS OF THE LCA – additional impact categories according to EN 15804+A2-optional:
1000 kg Iron Hydroxide Yellow Pigment
Parameter Unit A1-A3 A1 A2 A3
Disease
Incidence of disease due to PM emissions (PM) ND ND ND ND
incidence
Human exposure efficiency relative to U235 (IR) kBq U235 eq ND ND ND ND
Comparative toxic unit for ecosystems (ETP-fw) CTUe ND ND ND ND
5 Environmental Product Declaration - Lanxess Deutschland GmbH - Iron Hydroxide Yellow Pigment (FeOOH)
Comparative toxic unit for humans (carcinogenic) (HTP-c) CTUh ND ND ND ND
Comparative toxic unit for humans (noncarcinogenic) (HTP-nc) CTUh ND ND ND ND
Soil quality index (SQP) SQP ND ND ND ND
Disclaimer 1 – for the indicator “Potential Human exposure efficiency relative to U235”. This impact category deals mainly with the
eventual impact of low-dose ionizing radiation on human health of the nuclear fuel cycle. It does not consider effects due to possible
nuclear accidents, occupational exposure or radioactive waste disposal in underground facilities. Potential ionizing radiation from the
soil, radon and from some construction materials is also not measured by this indicator.
Disclaimer 2 – for the indicators “abiotic depletion potential for non-fossil resources”, “abiotic depletion potential for fossil resources”,
“water (user) deprivation potential, deprivation-weighted water consumption”, “potential comparative toxic unit for ecosystems”,
“potential comparative toxic unit for humans – cancerogenic”, “Potential comparative toxic unit for humans - not cancerogenic”,
“potential soil quality index”. The results of this environmental impact indicator shall be used with care as the uncertainties on these
results are high as there is limited experience with the indicator.
6. LCA: Interpretation
The product is evaluated below for the weighted average of the
five versions, namely compacted, powder, granulate and
micronized.
The largest share of the gross energy demand is attributed in
each case to the production of raw materials (A1) (approx.
21,600 MJ, 54 %). The transport of the raw materials requires
approx. 6 % of the energy expenditures (A2) in each case,
while the production process accounts for a share of 40 %.
The results of the different product types do not differ
significantly. In the Climate Change- total category, the variation
of the results is between 2-9 %. Only in individual
environmental categories they differ. The granulate pigments
are having an higher value in the Climate Change-biogenic
category, due to an increased waste content. Overall, the
micronized delivery form of the COLORTHERM® brand has the
most deviations from the weighted average. In particular, the
results differ in the categories Resource use - fossils and Water
use. The differences can be explained by variations in the
recipes. With the exception of the Colortherm® form, all
pigments are produced only from two raw materials, of which
one, iron sulfate is calculated as burden-free (pre-consumer
waste). For more details between the five delivery forms see
the appendix.
The environmental impact categories are significantly
influenced (at least 46 %) by the provision of raw materials In Module A3 (manufacturing process), the environmental
(module A1). The only exceptions is the category Climate impacts for all colors are essentially dominated by the use of
Change, Biogenic, where the greatest influence lies in the electricity and natural gas. The only exceptions are the
manufacturing processes (Module A3) or in the transport of the categories Climate Change, Biogenic and Water Removal
input materials (Module A2). Potential (WDP), which mainly reflect the incineration of
industrial waste or, in some delivery forms of the yellow
With the exception of the Climate Change, Land Use category, pigment, the use of compressed air.
the transportation processes do not have a significant impact
on the environmental impact of the products. The share of the When interpreting the results, it should be noted that various
manufacturing processes (A3) in the individual categories is assumptions and estimates were made. This mainly concerns
between 0 % and 48 % in all categories. In the impact category the transports to the plant. It can be assumed that the influence
Climate Change, biogenic, the influences is at 70 %. on the overall result is not significant even with variations in the
assumptions / estimates made, since transports do not have a
major influence.
7. Requisite evidence
According to PCR Part B no proofs are required.
8. References
6 Environmental Product Declaration - Lanxess Deutschland GmbH - Iron Hydroxide Yellow Pigment (FeOOH)
Standards
BPR Regulation
EN 934-1 Regulation (EU) No 528/2012 of the European Parliament and
DIN EN 934-1:2008-04, Admixtures for concrete, mortar, and of the Council of 22 May 2012 concerning the making available
grout - Part 1: Common requirements. on the market and use of the biocidal products (Text with EES
relevance)
EN 12878
DIN EN 12878:2014, Pigments for the coloring of building SCS Global Services
materials based on cement and/or lime -Specifications and Scientific Certification Systems.
methods of test. https://www.scsglobalservices.com/
EN 15804 German Waste Catalog Ordinance (AVV)
DIN EN 15804:2012-04+A1 2013, Sustainability of onstruction Ordinance on the European List of Waste, WasteCatalog
works – Environmental product declarations – Core rules for the Ordinance dated December 10, 2001 (GermanFederal Gazette
product category ofconstruction products. I p. 3379), last amended by Article 1of the Ordinance dated
June 30, 2020 (GermanFederal Gazette I p. 1533).
ISO 9001
DIN EN ISO 9001:2015, Quality management systems– CLP Regulation
Requirements. Regulation (EG) no. 1272/2008 of the European Parliament
and of the Council of December 16, 2008,on classification,
ISO 14001 labeling, and packaging of substances and mixtures, amending
DIN EN ISO 14001:2015, Environmental management and repealing Directives 67/548/EEC and 1999/45/EC,
systems - Requirements with guidance for use. andamending Regulation (EC) no. 1907/2006 (Official Journal L
353 dated December 31, 2008, p. 1–1355), last amended by
ISO 14021 Delegated Regulation (EU)2021/1962 of the Commission dated
DIN EN ISO 14021:2016, Environmental labels and August 12, 2021 (Official Journal L 400/16).
declarations – Self-declared environmental claims (Type II
environmental labeling). Ecoinvent database
Ecoinvent database version 3.8, 2021
ISO 14025
DIN EN ISO 14025:2011-10, Environmental labels and GaBi Professional database
declarations – Type III environmental declarations –Principles GaBi Professional database version 10.2, 2022
and procedures.
IBU 2021
ISO 18451-1 Institut Bauen und Umwelt e.V.: General guide for theEPD
DIN EN ISO 18451-1:2019, Pigments, dyestuffs, and program of the Institut Bauen und Umwelt e.V.(IBU). Version
extenders - Terminology - Part 1: General terms. 2.0, Berlin: Institut Bauen und Umwelte.V., 2021.www.ibu-
epd.com
ISO 50001
DIN EN ISO 50001:2018, Energy management systems - PCR part A
Requirements with guidance for use. Product category rules for building-related productsand
services. Part A: Calculation rules for the LCA andrequirements
Further literature for the background report, v. 2.0. Berlin:Institut Bauen und
Umwelt e.V. (publisher), 2021.
CPR Regulation
Regulation (EU) No 305/2011 of the European Parliament and PCR: Inorganic pigments in different versions
of the Council of March 2011, laying down harmonised Product category rules for building-related productsand
conditions for the marketing of construction products and services. Part B: Requirements for the EPD forinorganic
repealing Council Directive 89/106/EEC pigments in different versions, v.1.0. Berlin:Institut Bauen und
Umwelt e.V. (publisher), 2021.
ECHA
European Chemicals Agency: Candidate List of substances of
very high concern, 2022
7 Environmental Product Declaration - Lanxess Deutschland GmbH - Iron Hydroxide Yellow Pigment (FeOOH)
Publisher
Institut Bauen und Umwelt e.V. +49 (0)30 3087748- 0
Hegelplatz 1 info@ibu-epd.com
10117 Berlin www.ibu-epd.com
Germany
Programme holder
Institut Bauen und Umwelt e.V. +49 (0)30 3087748- 0
Hegelplatz 1 info@ibu-epd.com
10117 Berlin www.ibu-epd.com
Germany
Author of the Life Cycle Assessment
TÜV Rheinland Energy GmbH +49 (0)221 806 0
Am Grauen Stein 33 carbon@de.tuv.com
51105 Köln www.tuv.com
Germany
Owner of the Declaration
Lanxess Deutschland GmbH, BU Inorganic Pigments +49 221 8885 5179
Rheinuferstr. 7 - 9 uwe.hempelmann@lanxess.com
47829 Krefeld bayferrox.com
Germany
8 Environmental Product Declaration - Lanxess Deutschland GmbH - Iron Hydroxide Yellow Pigment (FeOOH)
