ENVIRONMENTAL PRODUCT DECLARATION
as per ISO 14025 and EN 15804+A2
Owner of the Declaration JANSEN AG
Publisher Institut Bauen und Umwelt e.V. (IBU)
Programme holder Institut Bauen und Umwelt e.V. (IBU)
Declaration number EPD-JAN-20230116-CBA1-EN
Issue date 20.10.2023
Valid to 19.10.2028
Janisol 2 EI30 door width x height: 1230mm x 2180mm
Jansen AG
www.ibu-epd.com | https://epd-online.com
General Information
Jansen AG Janisol 2 EI30 door width x height: 1230mm x
2180mm
Programme holder Owner of the declaration
IBU – Institut Bauen und Umwelt e.V. JANSEN AG
Hegelplatz 1 Industriestrasse 34
10117 Berlin 9463 Oberriet
Germany Switzerland
Declaration number Declared product / declared unit
EPD-JAN-20230116-CBA1-EN 1 m2 Jansen Janisol 2 EI30 with a grammage of 59.18 kg/m². The actual
reference size of the declared single leaf door has dimensions of width x
height: 1230 mm x 2180 mm.
This declaration is based on the product category rules: Scope:
Windows and doors , 01.08.2021 The environmental product declaration refers to a single leaf door type
(PCR checked and approved by the SVR) Jansen Janisol 2 EI30 in specific dimension width x height. The
characteristic values used for the system components Janisol 2 in the LCA
are provided by Jansen AG.
Issue date
The declared product is defined according to the profile series and product
20.10.2023
characteristics.
The location of the production site is Oberriet/ Switzerland.
Valid to
This EPD was created with the help of a semi-automatic LCA-Tool.
19.10.2028 The owner of the declaration shall be liable for the underlying information
and evidence; the IBU shall not be liable with respect to manufacturer
information, life cycle assessment data and evidences.
The EPD was created according to the specifications of EN 15804+A2. In
the following, the standard will be simplified as EN 15804.
Verification
The standard EN 15804 serves as the core PCR
Independent verification of the declaration and data according to ISO
14025:2011
Dipl.-Ing. Hans Peters internally X externally
(Chairman of Institut Bauen und Umwelt e.V.)
Florian Pronold Matthias Klingler,
(Managing Director Institut Bauen und Umwelt e.V.) (Independent verifier)
1 Environmental Product Declaration - Jansen AG - Janisol 2 EI30 door width x height: 1230mm x 2180mm
Product
According to the CE marking, the following structural data for
Product description/Product definition the element must be stated:
Jansen Janisol 2 is our fire-rated system for EI30 classifications
Constructional data
and fulfills very high safety requirements. With 60mm
construction depth, it is compatible with our other (non-fire Name Value Unit
protection) window and door series. Combinations with burglar Resistance to wind load acc. to EN
4 class
resistance, bullet resistance or emergency exits in public 12210
buildings are visually identical and can be excellently integrated Water tightness acc. to EN 12208 4A class
into the building envelope without offsets or visual losses. The
Sound insulation class according to EN Rw 43 db
performance of the system has been internationally confirmed -
ISO 10140 (-2;-5)
in numerous fire tests in combination with many different makes
Heat transfer coefficient acc. to DIN EN
of glass. 1.5 W/(m2K)
ISO 10077-2
This declaration describes the following element in Janisol 2: Air permeability acc. to EN 12207 4 class
Product: Jansen Janisol 2 EI30, single leaf door Classification of strength requirements
4 class
Face width: 132.5mm acc. to EN 1192
Construction depth: 60mm Mechanical durability acc. to EN 1191 /
8 class
Width x height: 1230mm x 2180mm EN 1603
CE marking according to EN 14351-1 Operating forces acc. to EN 13115 2 class
Fire resistance class acc. to DIN EN
For the placing on the market in the the European Union/ EI30 class
1634-1 / EN13501-2
European Free Trade Association EU/EFTA the CPR (EU) No.
Burglar protection class acc. to EN 1627 3 class
305/2011/ applies. The products require a declaration of
performance taking into account the harmonized product Product according to the CPR, based on an EN: Performance
standard EN 14351-1 windows and doors and a CE marking. data of the product in accordance with the declaration of
The respective national regulations apply to the use. With this performance with respect to its essential characteristics
declaration the following element is declared: according to EN 14351-1, doors. Other constructional data are
not relevant for this product.
Base materials/Ancillary materials
JANSEN Janisol 2 EI30 door is made of the following materials:
• Glazing approx. 48%
• Steel approx. 34%
• Gypsum board approx. 9%
• Plastics and fillers approx. 6%
• Fittings <2%
• Aluminium < 2%
• Stainless steel < 1%
The percentages relate to the most frequently sold product with
an opening of 2.68 m2. The percentages stated may vary
depending on the product type and dimensions.
Does the product or at least one part product contain materials
from the ECHA candidate list of materials which are especially
problematic for approval: Substances of Very High Concern –
SVHC (date 17.01.2023) above a mass % of 0.1: no.
This product/article/at least one partial article contains other
carcinogenic, mutagenic, reprotoxic (CMR) substances in
categories 1A or 1B which are not on the candidate list,
exceeding 0.1 percentage by mass: no.
Biocide products were added to this construction product or it
has been treated with biocide products (this then concerns a
treated product as defined by the (EU) Ordinance on Biocide
Products No. 528/2012): no.
Application
The Jansen Janisol 2 EI30 door can be integrated for building Reference service life
ventilation and light transmission and it meets all the
According to SBR 2011 regarding the specific material
requirements of an interior or exterior wall without taking over
characteristics of steel windows and doors, the reference
load-bearing functions.
service life is 75 years (SBR 2011). The practical service life
may well be longer. Conditions for a long service life are regular
Technical Data
maintenance, care and upkeep of the product. The specified
2 Environmental Product Declaration - Jansen AG - Janisol 2 EI30 door width x height: 1230mm x 2180mm
service life is independent of the manufacturer's warranty.
LCA: Calculation rules
Module C2 - considers 50 km truck transport to waste
Declared Unit processing. The transport distance can
The declared unit is a 1 m2 of Janisol 2 door element. be modified project-specific if required by linear scaling.
The actual reference size of the declared door element has
dimensions of 1230 mm x 2180 mm. Modules C3 and C4 - consider waste processing and/or
disposal with the following scenarios:
Declared unit
Name Value Unit • Scenario 1: 100% thermal treatment of all raw materials
with heating value including plastic system parts and
Declared unit 1 m2
100% recycling of metal system components (C3/1).
Grammage 59.18 kg/m2 Landfill of all materials without heating value (except
Layer thickness 0.06 m metals) including glazing (C4/1). For mineral based
components (i.e. gypsum board), construction waste
For inhomogeneous components made of different materials,
processing (shredding) and material recycling as filling
the conversion to other dimensions with factors leads to
material (incl. benefits for substitution of gravel in
deviations compared to the exact calculation. The frame
Module (D/1) is considered, assuming 3% recycling
percentage is 30.04% and the ground reference is 0.0738m².
losses are sent to landfill (C4/1).
Frame percentage = Frame surface / total area * 100 [%]
Ground reference = Element depth x element width [m²] • Scenario 2 (module C3/2): 100% recycling of plastic
system parts (excluding e-waste sent to incineration)
System boundary and 100% recycling of metal system components.
Type of EPD according to EN 15804: "cradle to gate with Landfill of all materials without heating value (except
options, modules C1–C4, and module D". The following metals) including glazing (C4/2). For mineral based
modules are declared: A1–A3, C, D and additional modules: components (i.e. gypsum board), construction waste
A4, A5 and B6. processing (shredding) and material recycling as filling
material (incl. benefits for substitution of gravel in
Production (modules A1-A3): Module D/2) are considered, assuming 3% recycling
losses are sent to landfill (C4/2).
This module considers the provision of all relevant door
components (i.e. metal profiles/components, plastic Modules C4/1 & C4/2 are identical.
parts/profiles and glazing) and raw materials including their
transport to the declared production plant. This considers the Benefits and loads beyond the product system boundary
manufacturing and assembly of these components, including (module D):
waste processing up to the end-of-waste state. The impact of
packaging materials is also covered by this module. Considers credits and loads from the recycling of the metal
components and mineral based components (i.e. gypsum
Transport to the construction site (module A4): board) as filling material (incl. benefits for the substitution of
gravel (duplicated in D/1 and D/2) and the recycling of the
A distance of 100 km is considered for the transport of the plastic system parts/profiles (D/2). Avoided burdens from the
packed finished product via truck. The transport distance can thermal treatment of all raw materials with heating value
be modified project-specific if required by linear scaling. (including plastic system parts/profiles) (D/1) and packaging
treatment (duplicated in D/1 and D/2) under European
Installation (module A5): conditions are considered. This affects only the rate of primary
materials (no secondary materials).
Treatment and disposal of packaging material is considered in
this module. Credits for potential avoided burdens due to Geographic Representativeness
energy substitution of electricity and thermal energy generation Land or region, in which the declared product system is
are declared in module D under European conditions and manufactured, used or handled at the end of the product´s
affects only the rate of primary materials (no secondary lifespan: Europe
materials).
Comparability
Operational energy use (module B6):
Electric consumption for operating the motorised door is Basically, a comparison or an evaluation of EPD data is only
considered. Its impacts are calculated per year. possible if all the data sets to be compared were created
according to EN 15804 and the building context, respectively
EoL stage (modules C1-C4): the product-specific characteristics of performance, are taken
into account. The following background database has been
Module C1 - considers manual deconstruction (without used for the LCA calculation: Sphera LCA software (GaBi ts)
environmental burdens). content update package (CUP) version 2022.2
LCA: Scenarios and additional technical information
2 door is declared below.
Characteristic product properties of biogenic carbon
Information on describing the biogenic Carbon Content at
No biogenic carbon is reported in the product. The biogenic
factory gate
carbon content in the accompanying packaging for 1 m2 Janisol
3 Environmental Product Declaration - Jansen AG - Janisol 2 EI30 door width x height: 1230mm x 2180mm
Name Value Unit 100% recycling of metal system components (C3/1). Landfill of
all materials without heating value (except metals) including
kg
Biogenic carbon content in product - glazing (C4/1). For mineral based components (i.e. gypsum
C
board), construction waste processing (shredding) and material
Biogenic carbon content in accompanying kg
0.0111 recycling as filling material (incl. benefits for substitution of
packaging C
gravel in Module D/1) are considered, assuming 3% recycling
Note: 1 kg of biogenic carbon is equivalent to 44/12 kg of CO . losses are sent to landfill (C4/1).
2
Scenario 2 considers 100% recycling of plastic system parts
(excluding e-waste sent to incineration) and 100% recycling of
The following technical information is a basis for the declared metal system components (C3/2). Landfill of all materials
modules. The values refer to the declared unit of 1 m2 of without heating value (except metals) including glazing (C4/2).
Jansen Janisol 2 EI30 door. For mineral based components (i.e. gypsum board),
construction waste processing (shredding) and material
Transport to the building site (A4)
recycling as filling material (incl. benefits for substitution of
Name Value Unit gravel in Module D/2) are considered, assuming 3% recycling
Litres of fuel 0.11 l/100km losses are sent to landfill (C4/2). Modules C4/1 and C4/2 are
Transport distance 100 km identical. The recycling of plastics scenario declared in this
EPD is currently considered a scenario that is not widely
Capacity utilisation (including empty runs) 61 %
available in reality due to economic viability limitations
Gross weight of packed products transported 59.21 kg
associated with higher costs of sorting smaller shares of
plastics such as those present in the declared product.
Installation into the building (A5)
Treatment and disposal of packaging material is considered in Name Value Unit
this module. EoL scenario 1 (modules C3/1 and C4/1)
The values refer to the declared unit of 1 m2 of Janisol 2 door. Collected separately waste type (door element) 59.18 kg
Name Value Unit Recycling (C3/1) 27.4 kg
Polyethylene (waste packaging to incineration) 0.00239 kg Energy recovery (C3/1) 2.74 kg
Cardboard box (waste packaging to incineration) 0.0115 kg Landfilling (C4/1) 29.18 kg
Wood (waste packaging to incineration) 0.0151 kg EoL scenario 2 (modules C3/2 and C4/2)
Collected separately (door element) 59.18 kg
According to SBR 2011 regarding the specific material
characteristics of steel windows and doors, the reference Recycling (C3/2) 30.0 kg
service life is 75 years (SBR 2011). The practical service life Energy recovery (C3/2) 0.14 kg
may well be longer. Conditions for a long service life are regular Landfilling (C4/2) 29.18 kg
maintenance, care and upkeep of the product. The specified
Reuse, recovery and/or recycling potentials (D), relevant
service life is independent of the manufacturer's warranty.
scenario information
Reference service life
Name Value Unit Module D includes the credits and loads from the recycling of
Life Span (according to SBR 2011) 75 a the metal components and mineral based components (i.e.
gypsum board) as filling material (incl. benefits for substitution
Operational energy use (B6) of gravel (duplicated in D/1 and D/2) and the recycling of the
The value below refers to the declared unit of 1 m2 of Jansen plastic system parts/profiles (D/2). Avoided burdens from the
Janisol 2 EI30 door. thermal treatment of all raw materials with heating value
(including plastic system parts/profiles) (D/1) and packaging
Name Value Unit
treatment (duplicated in D/1 and D/2) under European
Electricity consumption (per year) 72.39 MJ
conditions are considered. This affects only the rate of primary
materials (no secondary materials). A waste incineration plant
End of life (C1-C4)
with R1-value > 0.6 is assumed.
For the End-of-Life stage two scenarios are considered.
For recycling, a collection rate of 100% is considered.
Scenario 1 considers 100% thermal treatment of all raw
materials with heating value including plastic system parts and
4 Environmental Product Declaration - Jansen AG - Janisol 2 EI30 door width x height: 1230mm x 2180mm
LCA: Results
Results provided in this section are presented in relation to 1 m2 of door type Jansen Janisol 2 EI30 (reference dimensions 1230 mm x
2180 mm).
For the operational energy use (B6), electric consumption for operating the motorised door is considered. Its impacts are calculated per
year.
For the End-of-Life stage, two scenarios are considered:
C3/1 - considers 100% recycling of metal system components (duplicated in D/1 and D/2) and 100% thermal treatment of all raw
materials with heating value including plastic system parts. For mineral based components (i.e. gypsum board), construction waste
processing (shredding) and material recycling as filling material is considered.
C3/2 - considers 100% recycling of metal system components (duplicated in D/1 and D/2) and 100% recycling of plastic system parts
(excluding e-waste sent to incineration). For mineral based components (i.e. gypsum board), construction waste processing
(shredding) and material recycling as filling material is considered.
C4/1 and C4/2 - consider landfill of all materials without heating value (except metals) including glazing and recycling losses from
mineral based components (i.e. gypsum board). Modules C4/1 and C4/2 are identical.
D/1 - considers credits and loads from the recycling of the metal components and mineral based components (i.e. gypsum board) as
filling material (incl. benefits for the substitution of gravel (duplicated in D/1 and D/2). Avoided burdens from packaging treatment
(duplicated in D/1 and D/2) and thermal treatment of all raw materials with heating value (including plastic system parts/profiles) are
considered.
D/2 - considers credits and loads from the recycling of the metal components and mineral based components (i.e. gypsum board) as
filling material (incl. benefits for the substitution of gravel (duplicated in D/1 and D/2) and the recycling of the plastic system
parts/profiles. Avoided burdens from packaging treatment (duplicated in D/1 and D/2) are considered.
DESCRIPTION OF THE SYSTEM BOUNDARY (X = INCLUDED IN LCA; ND = MODULE OR INDICATOR NOT DECLARED; MNR =
MODULE NOT RELEVANT)
Benefits and
Construction loads beyond
Product stage Use stage End of life stage
process stage the system
boundaries
la ire ta m w a Ry lp p u s tro p s n a rT g n iru tc a fu n a M e h t m o rf tro p s n a rTe tis e h t o t e ta g y lb m e s s A e s U e c n a n e tn ia M ria p e R tn e m e c a lp e R tn e m h s ib ru fe R y g re n e la n o ita re p Oe s u re ta w la n o ita re p Oe s u n o itc u rts n o c -e Dn o itilo m e d tro p s n a rT g n is s e c o rp e ts a W la s o p s iD -e s u e R-y re v o c e R-g n ilc y c e Rla itn e to p
A1 A2 A3 A4 A5 B1 B2 B3 B4 B5 B6 B7 C1 C2 C3 C4 D
X X X X X MND MND MNR MNR MNR X MND X X X X X
RESULTS OF THE LCA - ENVIRONMENTAL IMPACT according to EN 15804+A2: 1 m2 Jansen Janisol 2 EI30 door (59.18
kg/m2)
Parameter Unit A1-A3 A4 A5 B6 C1 C2 C3/1 C3/2 C4/1 C4/2 D/1 D/2
GWP-total kg CO 2 eq 9.56E+01 3.57E-01 4.86E-02 8.3E+00 0 1.79E-01 6.56E+00 1.26E-01 4.38E-01 4.38E-01 -2.44E+01 -2.46E+01
GWP-fossil kg CO 2 eq 9.53E+01 3.54E-01 8.28E-03 8.29E+00 0 1.77E-01 6.56E+00 1.26E-01 4.35E-01 4.35E-01 -2.43E+01 -2.46E+01
GWP-
biogenic kg CO 2 eq 2.68E-01 1.49E-03 4.03E-02 4.9E-03 0 7.47E-04 3.59E-04 3.04E-05 1.47E-03 1.47E-03 -2.03E-02 -7.64E-03
GWP-luluc kg CO 2 eq 2.19E-02 1.98E-03 1.32E-07 5.38E-04 0 9.88E-04 7.65E-05 6.37E-05 8.04E-04 8.04E-04 -1.64E-03 -2.32E-03
kg CFC11
ODP 2.58E-10 2.12E-14 4.17E-15 8.19E-11 0 1.06E-14 4.54E-13 6.09E-14 1.02E-12 1.02E-12 -1.9E-11 -1.06E-11
eq
AP mol H+ eq 3.56E-01 3.37E-04 9.1E-06 1.22E-02 0 1.69E-04 2.32E-03 9.56E-05 3.09E-03 3.09E-03 -6.68E-02 -6.84E-02
EP-
kg P eq 1.07E-04 1.06E-06 1.13E-09 3.72E-06 0 5.29E-07 1.84E-07 6.76E-08 7.38E-07 7.38E-07 -8.58E-06 -7.61E-06
freshwater
EP-marine kg N eq 1.02E-01 1.05E-04 3.05E-06 3.33E-03 0 5.26E-05 1.04E-03 4.09E-05 7.89E-04 7.89E-04 -1.03E-02 -1.09E-02
EP-terrestrial mol N eq 1.19E+00 1.26E-03 4.22E-05 3.56E-02 0 6.31E-04 1.26E-02 4.78E-04 8.67E-03 8.67E-03 -9.86E-02 -1.05E-01
kg NMVOC
POCP 2.87E-01 2.94E-04 8.21E-06 9.4E-03 0 1.47E-04 2.71E-03 1.11E-04 2.4E-03 2.4E-03 -3.77E-02 -4.23E-02
eq
ADPE kg Sb eq 7.72E-03 2.96E-08 1.02E-10 9.86E-07 0 1.48E-08 2.55E-08 1.52E-08 4.46E-08 4.46E-08 -9.51E-05 -9.53E-05
ADPF MJ 1.15E+03 4.74E+00 1.15E-02 1.76E+02 0 2.37E+00 1.58E+00 3.28E-01 5.7E+00 5.7E+00 -2.61E+02 -3.18E+02
m3 world eq
WDP 4.79E+00 3.18E-03 5.54E-03 6.19E-01 0 1.59E-03 6.18E-01 2.55E-02 4.78E-02 4.78E-02 -4.14E+00 -3.99E+00
deprived
GWP = Global warming potential; ODP = Depletion potential of the stratospheric ozone layer; AP = Acidification potential of land and water; EP =
Eutrophication potential; POCP = Formation potential of tropospheric ozone photochemical oxidants; ADPE = Abiotic depletion potential for non-fossil
resources; ADPF = Abiotic depletion potential for fossil resources; WDP = Water (user) deprivation potential)
RESULTS OF THE LCA - INDICATORS TO DESCRIBE RESOURCE USE according to EN 15804+A2: 1 m2 Jansen Janisol 2 EI30
door (59.18 kg/m2)
Parameter Unit A1-A3 A4 A5 B6 C1 C2 C3/1 C3/2 C4/1 C4/2 D/1 D/2
PERE MJ 2.07E+02 2.69E-01 4.02E-01 2.54E+01 0 1.35E-01 2.9E-01 4.54E-02 8.56E-01 8.56E-01 -3.72E+01 -2.93E+01
PERM MJ 4E-01 0 -4E-01 0 0 0 0 0 0 0 0 0
PERT MJ 2.08E+02 2.69E-01 2.63E-03 2.54E+01 0 1.35E-01 2.9E-01 4.54E-02 8.56E-01 8.56E-01 -3.72E+01 -2.93E+01
5 Environmental Product Declaration - Jansen AG - Janisol 2 EI30 door width x height: 1230mm x 2180mm
PENRE MJ 1.06E+03 4.75E+00 1.22E-01 1.76E+02 0 2.37E+00 8.54E+01 8.41E+01 5.71E+00 5.71E+00 -2.61E+02 -3.19E+02
PENRM MJ 8.39E+01 0 -1.1E-01 0 0 0 -8.38E+01 -8.38E+01 0 0 0 0
PENRT MJ 1.15E+03 4.75E+00 1.15E-02 1.76E+02 0 2.37E+00 1.59E+00 3.29E-01 5.71E+00 5.71E+00 -2.61E+02 -3.19E+02
SM kg 1.28E+01 0 0 0 0 0 0 0 0 0 1.02E+01 1.15E+01
RSF MJ 0 0 0 0 0 0 0 0 0 0 0 0
NRSF MJ 0 0 0 0 0 0 0 0 0 0 0 0
FW m3 3.5E-01 3.05E-04 1.3E-04 3.85E-02 0 1.52E-04 1.45E-02 5.91E-04 1.45E-03 1.45E-03 -1.66E-01 -1.71E-01
PERE = Use of renewable primary energy excluding renewable primary energy resources used as raw materials; PERM = Use of renewable primary
energy resources used as raw materials; PERT = Total use of renewable primary energy resources; PENRE = Use of non-renewable primary energy
excluding non-renewable primary energy resources used as raw materials; PENRM = Use of non-renewable primary energy resources used as raw
materials; PENRT = Total use of non-renewable primary energy resources; SM = Use of secondary material; RSF = Use of renewable secondary fuels;
NRSF = Use of non-renewable secondary fuels; FW = Use of net fresh water
RESULTS OF THE LCA – WASTE CATEGORIES AND OUTPUT FLOWS according to EN 15804+A2:
1 m2 Jansen Janisol 2 EI30 door (59.18 kg/m2)
Parameter Unit A1-A3 A4 A5 B6 C1 C2 C3/1 C3/2 C4/1 C4/2 D/1 D/2
HWD kg 1.26E-07 2.27E-11 1.12E-12 1.26E-08 0 1.14E-11 1.62E-10 8.27E-12 2.93E-10 2.93E-10 4E-09 1.02E-09
NHWD kg 4.42E+00 6.81E-04 7.35E-04 3.74E-02 0 3.4E-04 7.93E-02 1.5E-02 2.92E+01 2.92E+01 3.77E-01 4.38E-01
RWD kg 3.38E-02 5.85E-06 6.55E-07 2.92E-02 0 2.92E-06 6.78E-05 8.71E-06 6.36E-05 6.36E-05 -7.82E-03 -4.59E-03
CRU kg 0 0 0 0 0 0 0 0 0 0 0 0
MFR kg 6.07E-01 0 0 0 0 0 2.74E+01 3E+01 0 0 0 0
MER kg 0 0 0 0 0 0 0 0 0 0 0 0
EEE MJ 0 0 5.55E-02 0 0 0 1.13E+01 1.28E-01 0 0 0 0
EET MJ 0 0 9.94E-02 0 0 0 2.03E+01 2.66E-01 0 0 0 0
HWD = Hazardous waste disposed; NHWD = Non-hazardous waste disposed; RWD = Radioactive waste disposed; CRU = Components for re-use;
MFR = Materials for recycling; MER = Materials for energy recovery; EEE = Exported electrical energy; EET = Exported thermal energy
RESULTS OF THE LCA – additional impact categories according to EN 15804+A2-optional:
1 m2 Jansen Janisol 2 EI30 door (59.18 kg/m2)
Parameter Unit A1-A3 A4 A5 B6 C1 C2 C3/1 C3/2 C4/1 C4/2 D/1 D/2
Disease
PM 3.58E-06 2.04E-09 4.78E-11 1.09E-07 0 1.02E-09 9.51E-09 1.96E-09 3.8E-08 3.8E-08 -8.06E-07 -8.12E-07
incidence
kBq U235
IR 5.32E+00 8.57E-04 1.07E-04 4.28E+00 0 4.29E-04 1.07E-02 1.19E-03 7.06E-03 7.06E-03 -1.15E+00 -5.61E-01
eq
ETP-fw CTUe 1.82E+03 3.29E+00 5.27E-03 5.39E+01 0 1.64E+00 7.21E-01 2.25E-01 3.2E+00 3.2E+00 -4.28E+01 -8.25E+01
HTP-c CTUh 8.99E-08 6.63E-11 3.46E-13 9.91E-10 0 3.31E-11 4.59E-11 5.56E-12 4.88E-10 4.88E-10 -9.96E-09 -1.1E-08
HTP-nc CTUh 3.44E-06 3.43E-09 1.3E-11 5.04E-08 0 1.71E-09 1.72E-09 2.73E-10 5.4E-08 5.4E-08 -3.14E-07 -3.86E-07
SQP SQP 2.07E+02 1.63E+00 3.32E-03 1.61E+01 0 8.15E-01 3.85E-01 8.4E-02 1.19E+00 1.19E+00 -8.51E+00 -5.2E+00
PM = Potential incidence of disease due to PM emissions; IR = Potential Human exposure efficiency relative to U235; ETP-fw = Potential comparative
Toxic Unit for ecosystems; HTP-c = Potential comparative Toxic Unit for humans (cancerogenic); HTP-nc = Potential comparative Toxic Unit for humans
(not cancerogenic); SQP = Potential soil quality index
Disclaimer 1 – for the indicator 'Potential Human exposure efficiency relative to U235'.This impact category deals mainly with the
eventual impact of low dose ionizing radiation on human health of the nuclear fuel cycle. It does not consider effects due to possible
nuclear accidents, occupational exposure or radioactive waste disposal in underground facilities. Potential ionizing radiation from the
soil, from radon and from some construction materials is also not measured by this indicator.
Disclaimer 2 – for the indicators 'abiotic depletion potential for non-fossil resources', 'abiotic depletion potential for fossil resources',
'water (user) deprivation potential, deprivation-weighted water consumption', 'potential comparative toxic unit for ecosystems', 'potential
comparative toxic unit for humans – cancerogenic', 'Potential comparative toxic unit for humans - not cancerogenic', 'potential soil
quality index'. The results of this environmental impact indicator shall be used with care as the uncertainties on these results are high
as there is limited experience with the indicator. This EPD was created using a software tool.
References
Standards ISO 14025
EN ISO 14025:2011, Environmental labels and declarations —
EN 14351-1 Type III environmental declarations — Principles and
EN 14351-1:2016, Windows and doors - Product standard, procedures.
performance characteristics - Part 1: windows and external
pedestrian doorsets EN 12210
EN 12210: 2016 Windows and doors - Resistance to wind
EN 16034 loads - classification
EN 16034:2014, pedestrian doorsets, industrial, commercial,
garage doors and openable windows - Product standard, EN 12208
performance characteristics - Fire resistance and/or smoke DIN EN 12208 Windows and doors - Watertightness -
control characteristics Classification
EN 15804 EN ISO 10140
EN 15804:2012+A2:2019+AC:2021, Sustainability of EN ISO 10140-1: 2021 Acoustics - Laboratory measurement of
construction works — Environmental Product Declarations — sound insulation of building elements - Part 1: Application
Core rules for the product category of construction products. rulesfor specific products
6 Environmental Product Declaration - Jansen AG - Janisol 2 EI30 door width x height: 1230mm x 2180mm
DIN EN ISO 10077-2 Authorisation (published in accordance with Article 59(10) ofthe
DIN EN ISO 10077-2: 2017 Thermal performance of windows, REACH Regulation)REGULATION (EU) No
doors and shutters - Calculation of thermal transmittance - 528/2012REGULATION (EU) No 528/2012 OF THE
Part2: Numerical method for frames EUROPEANPARLIAMENT AND OF THE COUNCIL, of 22 May
2012, concerning the making available on the market and use
EN 12207 of biocidal products
EN 12207: 2016 Windows and doors - Air permeability -
Classification SBR 2011
SBR life cycle guide [SBR 2011]
EN 1192
EN 1192: 2000 Doors - Classification of strength requirements Further References
EN 1191 Sphera LCA FE Software (GaBi ts)
EN 1191: 2012 Windows and doors - Resistance to repeated GaBi ts dataset documentation for the software-system and
opening and closing - Test method databases, LBP, University of Stuttgart and thinkstep,
Leinfelden-Echterdingen, 2023 (https://www.gabi-
EN 1603 software.com/support/gabi)
DIN EN 1603:2013-05 Thermal insulating products for building
applications - Determination of dimensional stability under Sphera LCA Calculator Software (GaBi Envision)
constant normal laboratory conditions GaBi Envision 5.0 Sphera Solution GmbH, the LCA, EPD and
Ecodesign tool, http://www.gabi-
EN 13115 software.com/international/software/gabi-envision/, 2022
EN 13115: 2020 Windows - Classification of mechanical
properties - Racking, torsion and operating forces.
DIN EN 1634-1 Jansen LCA tool
DIN EN 1634-1 Fire resistance and smoke control tests for door LCA tool for façades, windows & door
and shutter assemblies, openable windows and elements of LCA-Tool No.: IBU-JAN-202301-LT1-EN
building hardware - Part 1: Fire resistance test for door and Developed by Sphera Solutions GmbH
shutter assemblies and openable windows
IBU 2021
Institut Bauen und Umwelt e.V.: General Instructions for the
EN 13501-2 EPD programme of Institut Bauen und Umwelt e.V., Version
EN 13501-2: 2021 Fire classification of construction products 2.0, Berlin: Institut Bauen und Umwelt e.V., 2021
and building elements - Part 2: Classification using data from
fire resistance and/or smoke control tests, excluding ventilation www.ibu-epd.com
services
PCR Part A
EN 1627 PCR - Part A: Calculation rules for the Life Cycle Assessment
DIN EN 1627:2011-09 Pedestrian doorsets, windows, curtain and Requirements on the Background Report, version 1.3,
walling, grilles and shutters - Burglar resistance - Requirements Institut Bauen und Umwelt e.V., 08-2021.
and classification
ECHA candidate list PCR Part B
ECHA candidate list [BSJ1] - Substances of Very High PCR – Part B: Requirements on the EPD for Windows and
Concern– SVHC (date 17.01.2023) doors, version 1.6, Institut Bauen und Umwelt e.V., 2022
Candidate List of substances of very high concern for
7 Environmental Product Declaration - Jansen AG - Janisol 2 EI30 door width x height: 1230mm x 2180mm
Publisher
Institut Bauen und Umwelt e.V. +49 (0)30 3087748- 0
Hegelplatz 1 info@ibu-epd.com
10117 Berlin www.ibu-epd.com
Germany
Programme holder
Institut Bauen und Umwelt e.V. +49 (0)30 3087748- 0
Hegelplatz 1 info@ibu-epd.com
10117 Berlin www.ibu-epd.com
Germany
Author of the Life Cycle Assessment
Sphera Solutions GmbH +49 (0)711 341817-0
Hauptstraße 111- 113 info@sphera.com
70771 Leinfelden-Echterdingen www.sphera.com
Germany
Owner of the Declaration
JANSEN AG 0041717639113
Industriestrasse 34 sustainability@jansen.com
9463 Oberriet www.jansen.com
Switzerland
8 Environmental Product Declaration - Jansen AG - Janisol 2 EI30 door width x height: 1230mm x 2180mm
