ENVIRONMENTAL PRODUCT DECLARATION
as per ISO 14025 and EN 15804+A2
Owner of the Declaration dormakaba International Holding GmbH
Publisher Institut Bauen und Umwelt e.V. (IBU)
Programme holder Institut Bauen und Umwelt e.V. (IBU)
Declaration number EPD-DOR-20220214-CBA2-EN
Issue date 19.10.2022
Valid to 18.10.2027
Remote reader 91 15
dormakaba
www.ibu-epd.com | https://epd-online.com
General Information
dormakaba Remote reader 91 15
Programme holder Owner of the declaration
IBU – Institut Bauen und Umwelt e.V. dormakaba International Holding GmbH
Hegelplatz 1 DORMA Platz 1
10117 Berlin 58256 Ennepetal
Germany Germany
Declaration number Declared product / declared unit
EPD-DOR-20220214-CBA2-EN 1 piece of the product: Remote reader 91 15
This declaration is based on the product category rules: Scope:
Electronic and physical Access Control Systems, 01.08.2021 This EPD refers to a specific product manufactured by dormakaba. The
(PCR checked and approved by the SVR) production site is located in Villingen-Schwenningen (Germany).
The data represents the year 2020.
Issue date The owner of the declaration shall be liable for the underlying information
and evidence; the IBU shall not be liable with respect to manufacturer
19.10.2022
information, life cycle assessment data and evidences.
The EPD was created according to the specifications of EN 15804+A2. In
Valid to
the following, the standard will be simplified as EN 15804.
18.10.2027
Verification
The standard EN 15804 serves as the core PCR
Independent verification of the declaration and data according to ISO
14025:2011
internally X externally
Dipl.-Ing. Hans Peters
(Chairman of Institut Bauen und Umwelt e.V.)
Florian Pronold Dr.-Ing. Wolfram Trinius,
(Managing Director Institut Bauen und Umwelt e.V.) (Independent verifier)
1 Environmental Product Declaration - dormakaba - Remote reader 91 15
Product
Product description/Product definition Peripherals Interface
The dormakaba remote reader 91 15 offers the benefit of Variant MRD
separating the registration unit and door control unit. This • 2x coaxial for registration units (LEGIC / MIFARE)
makes it suitable for installation in protected internal areas to • 1x RS-485
control access points located in nonprotected external areas. • 1x RS-232
Thanks to its flexible integration, the dormakaba remote reader • 3x potential-free relays, 30 V AC/DC; max. 2 A
91 15 can be integrated into all dormakaba systems, whether • 4x digital inputs
online, CardLink or stand-alone operation. The control unit is • 1x tamper contact
typically positioned away from the registration unit, thereby
allowing wiring positioned close to the door. The communication Variant Wiegand
is encrypted, offering a high level of security. For the placing on • 2x Wiegand
the market in the European Union/European Free Trade • 1x RS232
Association (EU/EFTA) (with the exception of Switzerland) the • 3x potential-free relays, 30 V AC/DC; max. 2 A
following legal provisions apply: • 4x digital inputs
• Electromagnetic Compatibility Directive (EMC) • 1x tamper contact
• Low Voltage Directive (LVD)
• Restriction of Hazardous Substances (RoHS)
• Radio Equipment Directive (RED) Power supply
• EN 50581 • PoE, as per IEEE 802.3af
• PoE+, as per IEEE 802.3at
The CE-marking takes into account the proof of conformity with
the respective harmonized standards based on the legal Output voltage
provisions above. For the application and use the respective • Reader: 5/12 V DC • Elec. door opener: 12/24 V DC
national provisions apply.
Class of protection as per EN 60529:IP40.
Application
The dormakaba remote reader 91 15 is particularly suited for The product is not harmonised in accordance with the
external doors and access points that require a high level of Construction Product Regulations (CPR) but in accordance with
security. Depending on the function type, it supports different other provisions for harmonisation of the EU. Compliance with
systems and technologies and is available in various versions the European Union Directive and technical specifications:
and combinations of recording units. • EN 55032
• EN 55024+A1
Areas of application: • EN 50364
• External gates and gateways • EN 62368-1+A11
• Automatic doors • EN 60529
• Lifts • EN 301489-1 V2.2.1
• Garage doors • EN 301489-3 V2.1.1
• Car park barriers • EN 300330 V2.1.1
• Entrance areas
• Motor locks The product is subject to CE marking according to the relevant
harmonization legislation.
Technical Data In addition, the product also conforms to the
The Remote reader 91 15 has the following technical followingstandards:
properties:
• UL 294
Name Value Unit • UL 62368-1
Operating Temperature 0 - 50 °C • CAN/CSA-22.2 No. 62368-1
Operating Humidity 5 - 85 %
Base materials/Ancillary materials
Width Dimension 70 mm
The major material compositions of the product are listed
Height Dimension 106 mm
below:
Depth Dimension 45 mm
Name Value Unit
Weight (without packaging) 0,120 kg
Electronics 40 %
Weight (with packaging) 0,185 kg
Paper 36 %
Power consumption "idle mode" 2 W
Plastics 23 %
Power consumption "on mode" 5 W
The product includes partial articles which contain substances
Host Interface listed in the Candidate List of REACH Regulation
• Ethernet 10/100 Mbit/s 1907/2006/EC (date: 17.01.2022) exceeding 0.1 percentage by
mass in the alloy: no The Candidate List can be found on the
ECHA website address: https:echa.europa.eu/de/home.
Reference service life
The reference service life of the dormakaba Remote reader 91
15 is estimated to be 12 years. This number is based on the
support and service life and is not an estimated lifetime.
2 Environmental Product Declaration - dormakaba - Remote reader 91 15
LCA: Calculation rules
Declared Unit Use stage - Module B6
The declared unit is 1 piece of the product: Remote reader 91 The use stage related to the operation of the building includes:
15. — B6, operational energy use
Declared unit
End-of-life stage– Modules C1-C4 and D
Name Value Unit
The end-of-life stage includes:
Declared unit 1 pce.
— C1, de-construction, demolition:
Product weight including packaging 0,185 kg — C2, transport to waste processing;
— C3, waste processing for reuse, recovery and/or recycling;
System boundary — C4, disposal; including provision and all transport, provision
The type of EPD is: cradle to gate with options, modules C1– of all materials, products and related energy and water use.
C4, and module D (A1–A3 + C + D and additional modules: A4
+ A5 + B6)
Module D (Benefits and loads beyond the system boundary)
Production - Module A1-A3The product stage includes: includes:
— A1, raw material extraction, processing and mechanical — D, recycling potentials, expressed as net impacts and
treatments, processing of secondary material input (e.g. benefits.
recycling processes),
Geographic Representativeness
— A2, transport to the manufacturer,
Land or region, in which the declared product system is
— A3, manufacturing and assembly including provision of all
manufactured, used or handled at the end of the product´s
materials, products and energy, as well as waste processing up
lifespan: Germany
to the end-of waste state.
Construction stage - Modules A4-A5
Comparability
The construction process stage includes:
Basically, a comparison or an evaluation of EPD data is only
— A4, transport to the building site;
possible if all the data sets to be compared were created
— A5, installation into the building; including provision of all
according to EN 15804 and the building context, respectively
materials, products and energy, as well as waste processing up
the product-specific characteristics of performance, are taken
to the end-of-waste state or disposal of final residues during the
into account. Background database: GaBi, SP40.
construction process stage.
LCA: Scenarios and additional technical information
Operational energy use (B6) and Operational water use
Characteristic product properties of biogenic carbon
(B7)
Information on describing the biogenic Carbon Content at The use stage is declared for 15 years.
factory gate
Name Value Unit
Name ValueUnit
Energy consumption for 1 year 13,51 kWh
Biogenic carbon content in accompanying kg
0.02 on mode per day 2 h
packaging C
idle mode 22 h
Note: 1 kg of biogenic carbon is equivalent to 44/12 kg of CO .
2 on mode power 2 W
idle mode 1,5 W
Days per year in use 365 days
The following technical scenario information is required for the
declared modules.
End of life (C1-C4)
Transport to the building site (A4) C1: The product dismantling from the building is done manually
Name Value Unit without environmental burden.
Litres of fuel per 1 kg (truck) 0.00276 l/100km Name Value Unit
Transport distance via truck 100 km Collected separately waste type waste type 0.127 kg
Capacity utilisation (including empty runs) 55 % Recycling 0.071 kg
In order to allow scaling to a specific point of installation, 100 Energy recovery 0.043 kg
km are declared. Final deposition 0,013 kg
Transportation to Waste 50 km
Installation into the building (A5)
Region for end of life: Global
Name Value Unit
Waste Packaging (paper) 0.053 kg Reuse, recovery and/or recycling potentials (D), relevant
scenario information
Reference service life Collection rate is 100%.
Name Value Unit
Life Span according to the manufacturer 12 a
3 Environmental Product Declaration - dormakaba - Remote reader 91 15
LCA: Results
DESCRIPTION OF THE SYSTEM BOUNDARY (X = INCLUDED IN LCA; MND = MODULE OR INDICATOR NOT DECLARED; MNR
= MODULE NOT RELEVANT)
Benefits and
Construction loads beyond
Product stage Use stage End of life stage
process stage the system
boundaries
la ire ta m w a Ry lp p u s tro p s n a rT g n iru tc a fu n a M e h t m o rf tro p s n a rTe tis e h t o t e ta g y lb m e s s A e s U e c n a n e tn ia M ria p e R tn e m e c a lp e R tn e m h s ib ru fe R y g re n e la n o ita re p Oe s u re ta w la n o ita re p Oe s u n o itc u rts n o c -e Dn o itilo m e d tro p s n a rT g n is s e c o rp e ts a W la s o p s iD -e s u e R-y re v o c e R-g n ilc y c e Rla itn e to p
A1 A2 A3 A4 A5 B1 B2 B3 B4 B5 B6 B7 C1 C2 C3 C4 D
X X X X X MND MND MNR MNR MNR X MND X X X X X
RESULTS OF THE LCA - ENVIRONMENTAL IMPACT according to EN 15804+A2: 1 piece Remote reader 91 15
Parameter Unit A1-A3 A4 A5 B6 C1 C2 C3 C4 D
GWP-total kg CO 2 eq 1.24E-01 2E-03 7.6E-02 6.87E+01 0 2.45E-04 1.09E-01 1.91E-04 -8.3E-02
GWP-fossil kg CO 2 eq 2.26E-01 2E-03 2E-03 6.84E+01 0 2.34E-04 1.09E-01 1.9E-04 -8.3E-02
GWP-biogenic kg CO 2 eq -1.03E-01 6.96E-05 7.4E-02 2.11E-01 0 1.08E-05 2.54E-06 6.48E-07 -1.87E-04
GWP-luluc kg CO 2 eq 9.13E-04 3.58E-08 1.25E-06 9.4E-02 0 5.58E-09 6.16E-06 5.46E-07 -5.26E-05
ODP kg CFC11 eq 1.2E-10 1.59E-19 1.37E-17 1.41E-12 0 2.47E-20 5.5E-17 7.03E-19 -7.79E-16
AP mol H+ eq 5.19E-04 1.51E-06 2.12E-05 1.84E-01 0 2.35E-07 1.94E-05 1.36E-06 -1.12E-04
EP-freshwater kg P eq 2.24E-06 3.22E-10 2.67E-09 1.71E-04 0 5.01E-11 8.77E-09 3.26E-10 -9.74E-08
EP-marine kg N eq 1.79E-04 4.79E-07 7.67E-06 3.7E-02 0 7.46E-08 4.38E-06 3.5E-07 -2.93E-05
EP-terrestrial mol N eq 1.49E-03 5.33E-06 9.56E-05 3.96E-01 0 8.29E-07 8.84E-05 3.85E-06 -3.14E-04
kg NMVOC
POCP 5.26E-04 1.36E-06 2.03E-05 1.04E-01 0 2.11E-07 1.21E-05 1.06E-06 -8.5E-05
eq
ADPE kg Sb eq 1.43E-06 4.51E-11 2.16E-10 1.86E-05 0 7.03E-12 7.54E-10 1.7E-11 -5.89E-08
ADPF MJ 4.86E+00 2.1E-02 2.4E-02 1.17E+03 0 3E-03 5.1E-02 2E-03 -1.39E+00
m3 world eq
WDP 5.6E-02 2.95E-06 9E-03 1.49E+01 0 4.59E-07 1.1E-02 1.99E-05 -8E-03
deprived
GWP = Global warming potential; ODP = Depletion potential of the stratospheric ozone layer; AP = Acidification potential of land and water; EP =
Eutrophication potential; POCP = Formation potential of tropospheric ozone photochemical oxidants; ADPE = Abiotic depletion potential for non-fossil
resources; ADPF = Abiotic depletion potential for fossil resources; WDP = Water (user) deprivation potential)
RESULTS OF THE LCA - INDICATORS TO DESCRIBE RESOURCE USE according to EN 15804+A2: 1 piece Remote reader 91
15
Parameter Unit A1-A3 A4 A5 B6 C1 C2 C3 C4 D
PERE MJ 5.81E+00 6.73E-05 6.46E-01 5E+02 0 1.05E-05 1.63E-01 3.26E-04 -2.77E-01
PERM MJ 7.92E-01 0 -6.42E-01 0 0 0 -1.5E-01 0 0
PERT MJ 6.6E+00 6.73E-05 4E-03 5E+02 0 1.05E-05 1.3E-02 3.26E-04 -2.77E-01
PENRE MJ 3.19E+00 2.1E-02 2.4E-02 1.17E+03 0 3E-03 1.72E+00 2E-03 -1.39E+00
PENRM MJ 1.67E+00 0 0 0 0 0 -1.67E+00 0 0
PENRT MJ 4.86E+00 2.1E-02 2.4E-02 1.17E+03 0 3E-03 5.1E-02 2E-03 -1.39E+00
SM kg 0 0 0 0 0 0 0 0 0
RSF MJ 0 0 0 0 0 0 0 0 0
NRSF MJ 0 0 0 0 0 0 0 0 0
FW m3 1.7E-03 1.21E-07 2.21E-04 5.92E-01 0 1.88E-08 2.67E-04 6.28E-07 -3.23E-04
PERE = Use of renewable primary energy excluding renewable primary energy resources used as raw materials; PERM = Use of renewable primary
energy resources used as raw materials; PERT = Total use of renewable primary energy resources; PENRE = Use of non-renewable primary energy
excluding non-renewable primary energy resources used as raw materials; PENRM = Use of non-renewable primary energy resources used as raw
materials; PENRT = Total use of non-renewable primary energy resources; SM = Use of secondary material; RSF = Use of renewable secondary fuels;
NRSF = Use of non-renewable secondary fuels; FW = Use of net fresh water
RESULTS OF THE LCA – WASTE CATEGORIES AND OUTPUT FLOWS according to EN 15804+A2:
1 piece Remote reader 91 15
Parameter Unit A1-A3 A4 A5 B6 C1 C2 C3 C4 D
HWD kg 9.63E-07 2.07E-12 3.53E-11 4.91E-07 0 3.23E-13 1.93E-10 3.79E-11 -1.7E-09
NHWD kg 4.01E-03 2.18E-06 2E-03 8.05E-01 0 3.4E-07 1.1E-02 1.3E-02 -5.02E-04
RWD kg 8.6E-05 2.29E-08 1.26E-06 1.7E-01 0 3.57E-09 1.88E-06 2.83E-08 -9.47E-05
CRU kg 0 0 0 0 0 0 0 0 0
MFR kg 0 0 0 0 0 0 6.54E-04 0 0
MER kg 0 0 0 0 0 0 0 0 0
EEE MJ 0 0 1.15E-01 0 0 0 0 0 0
EET MJ 0 0 2.08E-01 0 0 0 0 0 0
4 Environmental Product Declaration - dormakaba - Remote reader 91 15
HWD = Hazardous waste disposed; NHWD = Non-hazardous waste disposed; RWD = Radioactive waste disposed; CRU = Components for re-use;
MFR = Materials for recycling; MER = Materials for energy recovery; EEE = Exported electrical energy; EET = Exported thermal energy
RESULTS OF THE LCA – additional impact categories according to EN 15804+A2-optional:
1 piece Remote reader 91 15
Parameter Unit A1-A3 A4 A5 B6 C1 C2 C3 C4 D
Disease
PM 4.21E-09 7.92E-12 1.18E-10 1.65E-06 0 1.23E-12 2.48E-10 1.68E-11 -9.69E-10
incidence
IR kBq U235 eq 1E-02 3.28E-06 1.95E-04 2.78E+01 0 5.1E-07 1.69E-04 2.91E-06 -1.6E-02
ETP-fw CTUe 2.26E+00 1.5E-02 1.1E-02 4.84E+02 0 2E-03 1.9E-02 1E-03 -2.75E-01
HTP-c CTUh 3.19E-10 2.85E-13 6.01E-13 1.37E-08 0 4.43E-14 1.64E-12 2.11E-13 -1.23E-11
HTP-nc CTUh 3.75E-09 1.22E-11 2.61E-11 5.1E-07 0 1.9E-12 1.66E-10 2.32E-11 -4.82E-10
SQP SQP 1.27E+01 5.48E-05 6E-03 3.59E+02 0 8.54E-06 1.5E-02 5.19E-04 -1.99E-01
PM = Potential incidence of disease due to PM emissions; IR = Potential Human exposure efficiency relative to U235; ETP-fw = Potential comparative
Toxic Unit for ecosystems; HTP-c = Potential comparative Toxic Unit for humans (cancerogenic); HTP-nc = Potential comparative Toxic Unit for humans
(not cancerogenic); SQP = Potential soil quality index
Disclaimer 1 – for the indicator IRP This impact category deals mainly with the eventual impact of low dose ionizing radiation on human
health of the nuclear fuel cycle. It does not consider effects due to possible nuclear accidents, occupational exposure nor due to
radioactive waste disposal in underground facilities. Potential ionizing radiation from the soil, from radon and from some construction
materials is also not measured by this indicator.
Disclaimer 2 – for the indicators ADPE, ADPF, WDP, ETP-fw, HTP-c, HTP-nc, SQP
The results of this environmental impact indicator shall be used with care as the uncertainties on these results are high or as there is
limited experience with the indicator. This EPD was created using a software tool.
References
CAN/CSA-22.2 No. 62368-1 EN 50581
CAN/CSA-22.2 No. 62368-1:2014, Audio/video, information and EN 50581:2012, Technicial documentation for the assessment
communication technologyequipment — Part 1: Safety of elctrical and electronic products with respect to the
requirements restrictions of hazardous substances
Electromagnetic Compatibility Directive (EMC) EN 55024+A1
Directive 2014/30/EU of the European Parliamant and of the EN 55024:2010+A1:2015, Information technology equipment -
Council of 26 February 2014 on the harmonisation of the laws Immunity characteristics - Limits and methods of measurement
of the Member States relating to electromagnetic compatibility
EN 55032
EN 15804 EN 55032:2015, Electromagnetic compatibility of multimedia
EN 15804+A2:2019+AC:2021, Sustainability of construction equipment - Emission Requirements
works — Environmental Product Declarations — Core rules for
the product category of construction products EN 60529
EN 60529:2014, Degrees of protection provided by enclosures
EN 300330 V2.1.1 (IP 20)
Short Range Devices (SRD) - Radio equipment in the
frequency range 9 kHz to 25 MHz and inductive loop systems in EN 62368-1+A11
the frequency range 9 kHz to 30 MHz - Harmonised Standard EN 62368-1:2014+A11:2017, Audio/video, information and
covering the essential requirements of article 3.2 of the communication technology equipment - Part 1: Safety
Directive 2014/53/EU requirements
EN 301489-1 V2.2.1 ISO 14025
ElectroMagnetic Compatibility (EMC) standard for radio DIN EN ISO 14025:2011-10, Environmental labels and
equipment and services - Part 1: Common technical declarations — Type III environmental declarations —
requirements - Harmonised Standard covering the essential Principles and procedures
requirements of article 3.1(b) of Directive 2014/53/EU and the
essential requirements of article 6 of Directive 2014/30/EU Low Voltage Directive (LVD)
Directive 2014/35/EU of the European Parliament and of the
EN 301489-3 V2.1.1 Council of 26 February 2014 on the harmonisation of the laws
ElectroMagnetic Compatibility (EMC) standard for radio of the Member States relating to the making available on the
equipment and services - Part 3: Specific conditions for Short- market of electrical equipment designed for use within certain
Range Devices (SRD) operating on frequencies between 9 kHz voltage limits
and 246 GHz - Harmonised standard covering the essential
requirements of article 3.1(b) of Directive 2014/53/EU Radio Equipment Directive (RED)
Directive 2014/53/EU of the European Parliament and of the
EN 50364 Council of 16 April 2014 on the harmonisation of the laws of the
EN 50364:2010, Limitation of human exposure to Member States relating to the making available on the market
electromagnetic fields from devices operating in the frequency of radio equipment and repealing Directive 1999/5/EC
range 0 Hz to 300 GHz, used in Electronic Article Surveillance
(EAS), Radio Frequency Identification (RFID) and similar Registration, Evaluation, Authorisation and Restriction of
applications Chemicals (REACH)
Regulation (EC) No 1907/2006 of the European Parliament and
5 Environmental Product Declaration - dormakaba - Remote reader 91 15
of the Council on the Registration, Evaluation, Authorisation GaBi ts documentation
and Restriction of Chemicals (REACH) GaBi life cycle inventory data documentation (https://www.gabi-
software.com/support/gabi/gabi-database-2020-lci-
Restriction of Hazardous Substances (RoHS) documentation/)
Directive on the restriction of the use of certain hazardous
substances in electrical and electronic equipment (RoHS), LCA-tool dormakaba
Directive (EU) No 2011/65 LCA tool, IBU-DOR-202102-LT1-EN. Developed by Sphera
Solutions GmbH
UL 294
UL 294:2013, Standard for Safety Access Control System Unit PCR Part A
PCR – Part A:
UL 62368-1 Calculation Rules for the Life Cycle As-sessment and
UL 62368-1:2014, Standard for Audio/video, information and Requirements on the Project Re-port according to EN
communication technology equipment - Part 1: Safety 15804+A2:2019, Version 1.0, Institut Bauen und Umwelt e.V.,
requirements www.ibu-epd.com
Further References PCR Part B
PCR – Part B: Requirements on the EPD for Building Hardware
IBU product, version 1.3, Institut Bauen und Umwelt e.V., www.ibu-
Institut Bauen und Umwelt e.V.: General Instructions for the epd.com, 2019.
EPDs programme of Institut Bauen und Umwelt e.V. Version
2.0., Berlin: Institut Bauen und Umwelt e.V., 2021. www.ibu-
epd.com
GaBi ts software
Sphera Solutions GmbH
Gabi Software System and Database for Life Cycle Engineering
1992-2020 Version 10.0.0.71 University of Stuttgart Leinfelden-
Echterdingen
6 Environmental Product Declaration - dormakaba - Remote reader 91 15
Publisher
Institut Bauen und Umwelt e.V. +49 (0)30 3087748- 0
Hegelplatz 1 info@ibu-epd.com
10117 Berlin www.ibu-epd.com
Germany
Programme holder
Institut Bauen und Umwelt e.V. +49 (0)30 3087748- 0
Hegelplatz 1 info@ibu-epd.com
10117 Berlin www.ibu-epd.com
Germany
Author of the Life Cycle Assessment
Sphera Solutions GmbH +49 711 341817-0
Hauptstraße 111- 113 info@sphera.com
70771 Leinfelden-Echterdingen www.sphera.com
Germany
Owner of the Declaration
dormakaba International Holding GmbH +49 2333 793-0
DORMA Platz 1 info.de@dormakaba.com
58256 Ennepetal www.dormakaba.com
Germany
7 Environmental Product Declaration - dormakaba - Remote reader 91 15
