ENVIRONMENTAL PRODUCT DECLARATION
as per ISO 14025 and EN 15804+A1
Owner of the Declaration Stiferite
Publisher Institut Bauen und Umwelt e.V. (IBU)
Programme holder Institut Bauen und Umwelt e.V. (IBU)
Declaration number EPD-STF-20200241-CBA3-EN
Issue date 18.12.2020
Valid to 17.12.2025
Stiferite Pendenzato Class B average thickness
Stiferite
www.ibu-epd.com | https://epd-online.com
General Information
Stiferite Stiferite Pendenzato Class B average thickness
Programme holder Owner of the declaration
IBU – Institut Bauen und Umwelt e.V. Stiferite
Hegelplatz 1 Viale Navigazione Interna 54
10117 Berlin 35129 Padova
Germany Italy
Declaration number Declared product / declared unit
EPD-STF-20200241-CBA3-EN STIFERITE Pendenzato CLASS B is a composite panel made by a base
side by EPS and a top side based on Stiferite CLASS B, expanded rigid
polyurethane foam, covered on top side by bituminous glass fibres, and
produced by Stiferite. The EPD applies to 1 m2 of a average 122 mm thick
PUR sandwich board, i.e. 0.122 m3, with an average density between
foam and facing of 32.1 kg/m3.
This declaration is based on the product category rules: Scope:
Insulating materials made of foam plastics, 01.08.2021 Stiferite produces STIFERITE Pendenzato CLASS B is a composite panel
(PCR checked and approved by the SVR) made by a base side by EPS and a top side based on Stiferite CLASS B,
expanded rigid polyurethane foam, covered on top side by bituminous
glass fibres.The data have been provided by the only Stiferite factory that
Issue date was located in Padova (Italy) for the year 2019.The owner of the
declaration shall be liable for the underlying information and evidence; the
18.12.2020
IBU shall not be liable with respect to manufacturer information, life cycle
assessment data and evidences.
The owner of the declaration shall be liable for the underlying information
Valid to
and evidence; the IBU shall not be liable with respect to manufacturer
17.12.2025 information, life cycle assessment data and evidences.
The EPD was created according to the specifications of EN 15804+A1. In
the following, the standard will be simplified as EN 15804.
Verification
The standard EN 15804 serves as the core PCR
Independent verification of the declaration and data according to ISO
14025:2011
internally X externally
Dipl.-Ing. Hans Peters
(Chairman of Institut Bauen und Umwelt e.V.)
Dipl.-Ing. Hans Peters Prof. Dr. Birgit Grahl,
(Managing Director Institut Bauen und Umwelt e.V.) (Independent verifier)
1 Environmental Product Declaration - Stiferite - Stiferite Pendenzato Class B average thickness
Product
Name Value Unit
Product description/Product definition
Gross density 32.1 kg/m3
STIFERITE's thermo insulation panels are mainly used in the
building/construction sector or industrial insulation. Declared Average Thermal conductivity PU:0.027, W/mK
λD acc. to /EN 13165/ EPS:0.033
The panels are made of thermo-setting closed cells Compressive strength at 10%
> 150 kPa
polyurethane foam (PU) supplied with various types of flexible deformation acc. to /EN 826/
facers on both sides of the panel. The nature/type of facer Tensile strength perpendicular to the
> 40 kPa
contributes to the performance characteristics of the product face acc. to /EN 1607/
and its application.
Water absorption by total immersion Vol.-
< 2
acc. to /EN 12087/ %
Expanded rigid polyurethane foam is distinguished by its good
Water absorption by partial immersion
thermo insulation performance, mechanical resistance, < 0.1 kg/m²
acc. to /EN 1609/
workability, lightness, and durability.
Water vapour diffusion resistance PU:33, EPS:30-
factor μ acc. to /EN 12086/ 70
The performance of STIFERITE's panels is determined based
on the European norm EN 13165:2012+A2:2016 Thermal Euroclass reaction to fire acc. to /EN
F
insulation products for buildings - Factory made rigid 11925/
polyurethane foam (PU) products - Specification for
This provides a thermal resistance R = 4.14 m² k/W.
polyurethane insulation board and on the European norm EN
13163:2012+A2:2016 Thermal insultaion for building-factory
The LCI data used in this report refer to an average product
made expanded polystyrene (EPS) products - Specification for
having an average thickness (materials in the recipes of
polystyrene insulation board.
different thicknesses are weighted according to the relative
This EPD refers to STIFERITE PENDENZATO CLASS B
production in square meters). The type of declaration is 1 c -
Average thick panel, made of an insulation component in
declaration of an average product from a manufacturer's plant.
polyurethane foam using blowing agent Pentane-based,
covered on top side by bituminous glass fibers, and on the
bottom side of an insulation component in EPS with a slope
shape. Base materials/Ancillary materials
PU insulation panel (about 53,1 % of the weight of the
The panel is produced in standard dimensions of as request by declared unit):
the customers and straight finish borders. The surface of the Closed-cell Polyiso (PIR) rigid foam made from MDI (50-65%),
panel may be evened off by sandpaper in order to allow polyols (20-30 %), pentane (4-5%) and additives (4-7%).
installation to uneven surfaces. STIFERITE PENDENZATO PU Facing (about 14,6 % of the weight of the declared unit):
CLASS B Average thick panel is produced by a certified upper and lower facing consisting of bitumen (40-60 %), PP (4-
company with systems: 10 %), urea-formaldehyde (1-5 %), calcium carbonate (1-5%)
ISO 9001, ISO 45001, ISO 14001 in its entire line of products. and glass fibre (30-40 %).
For the placing on the market of the product in the
EuropeanUnion/European Free Trade Association (EU/EFTA) EPS insulation panels: about 32,3 % The PU board for
(with the exception of Switzerland) Regulation (EU) No. insulation:
305/2011 (CPR) applies. The product needs a declaration of
• This product/article/at least one partial article contains
perfomance taking into consideration for polyurethane side EU
substances listed in the candidate list (date: 17.11.2020)
13165:2012+A2:2016 Thermal insultaion for building-factory
exceeding 0.1 percentage by mass: no
made rigid polyurethane foam (PU) products – Specification
• This product/article/at least one partial article doesn't
and the CE marking, and for EPS side
contain other CMR substances in categories 1A or 1B
EN 13163:2012+A2:2016 Thermal insultaion for building-factory
which are not on the candidate list, exceeding 0.1
made expanded polystyrene (EPS) products– Specification and
percentage by mass: no
the CE marking. For the application and use the respective
• Biocide products were added to this construction
national provisions apply.
product or it has been treated with biocide products (this
Application then concerns a treated product as defined by the (EU)
Ordinance on Biocide Products No. 528/2012): no
The STIFERITE Pendenzato CLASS B panel is suited for roofs
Additional declaration according to quoted law: The product is
under bituminous waterproofing mantles and where high
compliant with all requirements indicated at chapter 2.5.7
resistance to a flame torch is required.
'Isolanti termici ed acustici' of the n.256 D.L. of the 23th June
Technical Data 2022 (CAM EDILIZIA):
The data provided by the Declaration of Performance apply. In • Any blowing agent with Ozone depletion potential >0 is
this Life Cycle Assessment, a PU insulation board with the not used in production
following properties has been regarded: • Any substances of Very High Concern-SVHC in
Constructional data concentration of more than 0,1 %w are not used in
production (REACH n. 1907/2006). Any specific
authorizations for use are eserved provided for by the
same Regulation for the substances included in Annex
XIV and specifications restrictions set out in Annex XVII
of the Regulation.
• Catalysts lead-based are not used in production
2 Environmental Product Declaration - Stiferite - Stiferite Pendenzato Class B average thickness
• Flame retardants used in production (belonging to the 4 %w (note: this information is not explicitly considered
Organophosphorus class) are not banned by any in the LCA and not included in the EPD tables that only
national or European regulation refer to recycling content in the foreground system).
• According to the raw materials declarations of suppliers
the minimum amount of recycled raw materials based Reference service life
on the EPS insulation weight is more than 15% and The durability of insulation panels is normally at least as long as
based on the insulation board (PU foam and facers) the lifetime of the building in which it is used. The experimental
weight is 3 %w and the minimum amount of recycled data show that the reference life is longer than 50 years, Clima
raw materials based on the PU insulation foam weight is 2019.
LCA: Calculation rules
This life cycle assessment for the production of the
Declared Unit polyurethane insulation board considers the life cycle from the
The declared unit is 1 m² with an average thickness of 122 mm, supply of raw materials to the manufacturer´s gate (cradle-to-
e. g. 0.122 m³. Corresponding conversion factors are listed in gate with options). It also includes the transport to the
the table below. construction site, the installation and the end-of-life stage of the
Declared unit used PU thermal insulation board. The life cycle is split into the
following individual phases:
Name Value Unit
A1 - Raw material formulation
Declared unit 1 m2 A2 - Raw material transport
Gross density 32.1 kg/m3 A3 - Production of the insulation board and packaging material
Volume 0.122 m³ A4 - Transport to the construction site
A5 - Emissions and cutting losses during installation and
Grammage 392 kg/m2
packaging disposal
Declared average thermal PU:0.027, W/mK C2 - Transport to end-of-life
conductivity λD EPS:0.033 C3/C4 - End-of-Life: waste management (thermal recovery,
Layer thickness 0.122 m landfill)
Conversion factor to 1 kg 3.92 kg/m² D - Benefits and loads beyond system boundary
Weight of declared unit 3.92 kg/m²
Geographic Representativeness
This provides a thermal resistance R = 4.14 m² /W. Land or region, in which the declared product system is
manufactured, used or handled at the end of the product´s
The LCI data used in this report refer to an average product lifespan: Italy
having an average thickness (materials in the recipes of
different thicknesses are weighted according to the relative
production in square meters). The type of declaration is 1 c - Comparability
declaration of an average product from a manufacturer's plant. Basically, a comparison or an evaluation of EPD data is only
possible if all the data sets to be compared were created
according to EN 15804 and the building context, respectively
the product-specific characteristics of performance, are taken
System boundary into account. For life cycle modelling of the considered
products, the GaBi 9 2020 has been used.
LCA: Scenarios and additional technical information
End of life (C1-C4)
The results for the end-of-life are declared for the 2 different
Transport to the building site (A4) scenarios:
The distances calculated are weighted average distances Name Value Unit
according to the overall sales distribution; such distribution is
Scenario No 1: Material Incineration 100 %
considered similar for all Stiferite products.
Scenario No 2: Landfill 100 %
Name ValueUnit
C4: Disposal scenarios used is divided into the 2
Truck with a capacity of 17.3 tons 270 km
sub-scenarios:
Ferry with a capacity of 1200-10000 dwt payload
124 km 1) Incineration 100% (C4/1)
capacity
2) Landfilling 100% (C4/2)
Ship with a capacity of 27500 dwt payload capacity
11000 km
tons D: Benefits and loads beyond system boundary are divided into
Plane with a capacity of 22 ton 0 km the 2 sub-scenarios:
1) Incineration 100% (D1)
Installation into the building (A5) 2) Landfilling 100% (D2)
Name Value Unit
Material loss 0.0784 kg
VOC in the air Pentane 1.27E-06 kg
3 Environmental Product Declaration - Stiferite - Stiferite Pendenzato Class B average thickness
LCA: Results
The tables below show the results of the LCA. There are two scenarios for the end-of-life (C3, C4 and D) analyzed: Scenario 1
considers 100% incineration, Scenario 2 considers 100% landfill disposal.
For (SM, RSF, NRSF,CRU) indicators only the foreground system is considered.
DESCRIPTION OF THE SYSTEM BOUNDARY (X = INCLUDED IN LCA; MND = MODULE NOT DECLARED; MNR = MODULE NOT
RELEVANT)
Benefits and
Construction loads beyond
Product stage Use stage End-of-life stage
process stage the system
boundaries
la ire ta m w a Ry lp p u s tro p s n a rT g n iru tc a fu n a M e h t m o rf tro p s n a rTe tis e h t o t e ta g y lb m e s s A e s U e c n a n e tn ia M ria p e R tn e m e c a lp e R tn e m h s ib ru fe R y g re n e la n o ita re p Oe s u re ta w la n o ita re p Oe s u n o itc u rts n o c -e Dn o itilo m e d tro p s n a rT g n is s e c o rp e ts a W la s o p s iD -e s u e R-y re v o c e R-g n ilc y c e Rla itn e to p
A1 A2 A3 A4 A5 B1 B2 B3 B4 B5 B6 B7 C1 C2 C3 C4 D
X X X X X MND MND MNR MNR MNR MND MND MND X X X X
RESULTS OF THE LCA - ENVIRONMENTAL IMPACT according to EN 15804+A1: 1 m² PENDENZATO CLASS B average
thickness panel
Parameter Unit A1-A3 A4 A5 C2 C3/1 C3/2 C4/1 C4/2 D/1 D/2
GWP kg CO 2 eq 9.72E+00 7.36E-02 2.51E-01 1.84E-02 0 0 7.88E+00 4.46E-01 -3.79E+00 -4.42E-02
ODP kg CFC11 eq 1E-05 1.62E-17 2E-07 4.57E-18 0 0 5.53E-15 3.68E-15 -6.84E-14 -6.24E-16
AP kg SO 2 eq 2.22E-02 6.69E-04 4.94E-04 4.04E-05 0 0 3.02E-03 8.86E-04 -5.61E-03 -5.47E-05
EP kg PO 43 eq 2.86E-03 8.97E-05 6.99E-05 9.81E-06 0 0 6.14E-04 3.24E-04 -6.74E-04 -7.35E-06
POCP kg Ethen eq 1.25E-02 -1.27E-05 2.52E-04 -1.3E-05 0 0 1.77E-04 7.05E-05 -4.73E-04 -6.38E-06
ADPE kg Sb eq 3.39E-05 5.64E-09 6.87E-07 1.69E-09 0 0 3.82E-07 1.58E-07 -8.44E-07 -1.02E-08
ADPF MJ 2.52E+02 9.77E-01 5.24E+00 2.49E-01 0 0 4.24E+00 3.35E+00 -5.14E+01 -1.06E+00
GWP = Global warming potential; ODP = Depletion potential of the stratospheric ozone layer; AP = Acidification potential of land and water; EP =
Eutrophication potential; POCP = Formation potential of tropospheric ozone photochemical oxidants; ADPE = Abiotic depletion potential for non-fossil
resources; ADPF = Abiotic depletion potential for fossil resources
RESULTS OF THE LCA - INDICATORS TO DESCRIBE RESOURCE USE according to EN 15804+A1: 1 m² PENDENZATO CLASS
B average thickness panel
Parameter Unit A1-A3 A4 A5 C2 C3/1 C3/2 C4/1 C4/2 D/1 D/2
PERE MJ 1.16E+01 IND 2.66E-01 IND IND IND 1.32E+00 IND IND IND
PERM MJ 0 IND 0 IND IND IND 0 IND IND IND
PERT MJ 1.16E+01 4.46E-02 2.66E-01 1.44E-02 0 0 1.32E+00 9.56E-01 -1.82E+01 -1.36E-01
PENRE MJ 1.19E+02 IND 1.94E+00 IND IND IND 1.48E+02 IND IND IND
PENRM MJ 1.44E+02 IND -1.72E+00 IND IND IND -1.43E+02 IND IND IND
PENRT MJ 2.63E+02 9.81E-01 2.21E-01 2.5E-01 0 0 5.21E+00 4.04E+00 -6.7E+01 -1.14E+00
SM kg 0 0 0 0 0 0 0 0 0 0
RSF MJ 0 0 0 0 0 0 0 0 0 0
NRSF MJ 0 0 0 0 0 0 0 0 0 0
FW m3 6.09E-02 5.25E-05 1.36E-03 1.68E-05 0 0 1.97E-02 1.06E-03 -2.1E-02 -1.87E-04
PERE = Use of renewable primary energy excluding renewable primary energy resources used as raw materials; PERM = Use of renewable primary
energy resources used as raw materials; PERT = Total use of renewable primary energy resources; PENRE = Use of non-renewable primary energy
excluding non-renewable primary energy resources used as raw materials; PENRM = Use of non-renewable primary energy resources used as raw
materials; PENRT = Total use of non-renewable primary energy resources; SM = Use of secondary material; RSF = Use of renewable secondary fuels;
NRSF = Use of non-renewable secondary fuels; FW = Use of net fresh water
RESULTS OF THE LCA – WASTE CATEGORIES AND OUTPUT FLOWS according to EN 15804+A1:
1 m² PENDENZATO CLASS B average thickness panel
Parameter Unit A1-A3 A4 A5 C2 C3/1 C3/2 C4/1 C4/2 D/1 D/2
HWD kg 1.06E-03 3.53E-08 2.11E-05 1.16E-08 0 0 9.71E-09 1.52E-08 -2.65E-08 -3.77E-10
NHWD kg 2.01E-01 1.43E-04 9.82E-02 3.97E-05 0 0 7.72E-01 3.88E+00 -3.36E-02 -3.58E-04
RWD kg 4.39E-03 1.65E-06 9.96E-05 4.61E-07 0 0 3.82E-04 2.72E-04 -6.2E-03 -3.47E-05
CRU kg 0 0 0 0 0 0 0 0 0 0
MFR kg 0 0 1.37E-02 0 0 0 0 0 0 0
MER kg 0 0 1.56E-02 0 0 0 3.92E+00 0 0 0
EEE MJ 0 0 8.65E-02 0 0 0 2.06E+01 0 0 0
EET MJ 0 0 1.56E-01 0 0 0 1.96E+01 0 0 0
HWD = Hazardous waste disposed; NHWD = Non-hazardous waste disposed; RWD = Radioactive waste disposed; CRU = Components for re-use;
MFR = Materials for recycling; MER = Materials for energy recovery; EEE = Exported electrical energy; EET = Exported thermal energy
References
4 Environmental Product Declaration - Stiferite - Stiferite Pendenzato Class B average thickness
Standards
ISO 9001
EN 15804 ISO 9001:2015 Quality management
EN 15804:2012-04+A1 2013, Sustainability of construction
works — Environmental Product Declarations — Core rules for ISO 14001
the product category of construction products. ISO 14001: 2015 Environmental management systems
ISO 14025 ISO 45001
DIN EN ISO 14025:2011-10, Environmental labels and ISO 45001: 2018 Occupational health and safety management
declarations — Type III environmental declarations — systems
Principles and procedures.
Further References
IBU 2016
Institut Bauen und Umwelt e.V.: General Programme BNB
Instructions for the Preparation of EPDs at the Institut Bauen Bewertungssystem Nachhaltiges Bauen (en: assessment
und Umwelt e.V. Version 1., Berlin: Institut Bauen und Umwelt system sustainable Building)
e.V., 2016. www.ibu-epd.com https://www.bbsr.bund.de/BBSR/EN/RP/FutureBuilding/2SustainableBuildingQuality/2009/ServiceLife/01_Start_dossier.html?
n=391866&notFirst=true&docId=390900
EN13163
EN 13163:2012+A2:2016 Thermal insultaion for building-factory Candidate List
made expanded polystyrene (EPS) products - Specification https://echa.europa.eu/it/candidate-list-table (date 17.11.2020)
EN 13165 Clima 2019
EN 13165:2012+A2:2016 Thermal insulation products for Clima 2019 PaperPolyurethane
buildings - Factory made rigid polyurethane foam (PU) 'Environmental Impacts for a Polyurethane Panel'
products - Specification E. Guolo, F. Cappelletti, P. Romagnoni, F. Raggiotto
EN 826 GaBi 9 2020
EN 826:2013 Determination of Compression Behavior of GaBi 9: Documentation of GaBi 9: Software-System and
Thermal Insulation Products Database for Life Cycle Engineering. Copyright, TM. Stuttgart,
Leinfelden-Echterdingen, 1992-2020
EN 1607 http://www.gabi-software.com
EN 1607: 2013 Thermal insulating products for building
applications. Determination of tensile strength perpendicular to PANGPP 2017
faces Piano d' Azione Nazionale sul Green Public Procurement
(PANGPP) – Gazzetta Ufficiale della Repubblica Italiana, Serie
EN 12087 Generale n.17, 11-10-2017,
EN 12087:2013 Thermal insulating products for building http://www.minambiente.it/sites/default/files/archivio/allegati/GPP/GPP_CAM_Edilizia.pdf
applications. Determination of long term water absorption by
immersion. PCR Part A
Product Category Rules for Building-Related Products and
EN 1609 Services.
EN 1609: Thermal insulating products for building applications. Part A: Calculation Rules for the Life Cycle Assessment and
Determination of short term water absorption by partial Requirements on the Background Report. Version 06.2017
immersion.
PCR Part B
EN 12086 PCR Guidance-Texts for Building-Related Products and
EN 12086:2013 Thermal insulating products for building Services; Part B: Requirements on the EPD for Insulating
applications. Determination of water vapour transmission materials made of foam plastics; Institute Construction and
properties. Environment e.V. (IBU). Version 06.2017
https://epd-online.com
EN 11925
EN 11925:2010 Reaction to fire tests. Ignitability of products REACH
subjected to direct impingement of flame. Single-flame source REACH Registration, Evaluation, Authorization and Restriction
test. of Chemical, 2007
5 Environmental Product Declaration - Stiferite - Stiferite Pendenzato Class B average thickness
Publisher
Institut Bauen und Umwelt e.V. +49 (0)30 3087748- 0
Hegelplatz 1 info@ibu-epd.com
10117 Berlin www.ibu-epd.com
Germany
Programme holder
Institut Bauen und Umwelt e.V. +49 (0)30 3087748- 0
Hegelplatz 1 info@ibu-epd.com
10117 Berlin www.ibu-epd.com
Germany
Author of the Life Cycle Assessment
thinkstep Italy +39 0544 467132
Via Bovini 43 info@thinkstep.com
48123 Ravenna www.thinkstep.com
Italy
Owner of the Declaration
Stiferite +39 049 8997911
Viale Navigazione Interna 54 info@stiferite.com
35129 Padova www.stiferite.com
Italy
6 Environmental Product Declaration - Stiferite - Stiferite Pendenzato Class B average thickness
