ENVIRONMENTAL PRODUCT DECLARATION
as per ISO 14025 and EN 15804+A2
Owner of the Declaration Hilti Aktiengesellschaft
Publisher Institut Bauen und Umwelt e.V. (IBU)
Programme holder Institut Bauen und Umwelt e.V. (IBU)
Declaration number EPD-HIL-20230211-IBC2-EN
Issue date 01.09.2023
Valid to 31.08.2028
MT- System (Outdoor)
HILTI AG
www.ibu-epd.com | https://epd-online.com
1. General Information
HILTI AG MT- System (Outdoor)
Programme holder Owner of the declaration
IBU – Institut Bauen und Umwelt e.V. Hilti Aktiengesellschaft
Hegelplatz 1 Feldkircher Strasse 100
10117 Berlin 9494 Schaan
Germany Liechtenstein
Declaration number Declared product / declared unit
EPD-HIL-20230211-IBC2-EN Name of declared product / declared unit
This declaration is based on the product category rules: Scope:
Connection, assembly and installation systems, 01.08.2021 This document relates to the I.-Girder MT-100 OC ('MT-100 OC”) as a
(PCR checked and approved by the SVR) representative product for the MT Outdoor profile portfolio. The MT
Outdoor profile portfolio is a set of installation channels and girders with 6
types of wall thickness –1.5mm, 1.75mm, 2mm, 2.75mm, 3mm and 4mm.
Issue date Then the products are distinguished into size classes by shape and load
performance. Each of these size classes are produced in 2 different
01.09.2023
lengths to accommodate intended use, which are 2 meters, 3 meters and 6
meters. The declared product for this EPD is MT-100 OC, with thickness of
4mm, because it is the worst case scenario within the MT Outdoor profile
Valid to
portfolio.
31.08.2028 The owner of the declaration shall be liable for the underlying information
and evidence; the IBU shall not be liable with respect to manufacturer
information, life cycle assessment data and evidences.
The EPD was created according to the specifications of EN 15804+A2. In
the following, the standard will be simplified as EN 15804.
Verification
The standard EN 15804 serves as the core PCR
Independent verification of the declaration and data according to ISO
14025:2011
Dipl.-Ing. Hans Peters internally X externally
(Chairman of Institut Bauen und Umwelt e.V.)
Florian Pronold Mrs Kim Allbury,
(Managing Director Institut Bauen und Umwelt e.V.) (Independent verifier)
1 Environmental Product Declaration - HILTI AG - MT- System (Outdoor)
2. Product
2.1 Product description/Product definition
The MT-100 OC is designed as a metallic substructure system
that is made of thin-walled steel in a rectangular shape with
surface coating for the outdoor environment. All 4 sides of the
profile with connection holes interfacs with other assembly
components to form a flexible modular support substructure
that is fastened to concrete or steel frame structures. They are
horizontal and vertical members at different lengths that
interconnect to form either 2D or 3D structures to carry the
weight and hold in place mechanical, electrical, and piping
services. For the placing of the product on the market in the
European Union European Free Trade Association/ EU/EFTA)
(with the exception of Switzerland) Regulation (EU) No.
305/2011 (CPR) applies. The product needs a declaration of
performance taking into consideration the following European
Technical Approval ETA-21/0414 assessed based on EAD
280016-00-0602 'Products for installation systems for
supporting technical building equipment' and the CE-marking.
For the application and use the respective national provisions
apply.
The individual channel items under this product family are as
listed below:
2 Environmental Product Declaration - HILTI AG - MT- System (Outdoor)
Name Value Unit
Thickness of material 4 mm
Height of profile 150 mm
Width of profile 100 mm
Length of profile 6000 mm
Performance data of the product in accordance with the
declaration of performance with respect to its essential
characteristics according to ETA-21/0414 assessed based on
EAD 280016-00-0602 'Products for installation systems for
supporting technical building equipment'.
2.4 Delivery status
The MT-100 OC is packaged in bundles of long goods, and
each length types are bundled together with steel straps then
protected at the edges with wooden blocks. The declared MT-
100 OC is delivered in 20 pieces of 6 meter lengths,
constituting a bundle of total 120 meters.
2.5 Base materials/Ancillary materials
Name ValueUnit
Continuously hot-dip zinc-magnesium alloy coated
100 %
steel
The raw material used to produce the declared product MT-100
OC is galvanized steel according to the standard EN
10346:2015, weighing 15.096 kg per meter.
This product/article/at least one partial article contains
substances listed in the REACH SVHC candidate list (date:
17.01.2023) exceeding 0.1 percentage by mass: NO.
This product/article/at least one partial article contains other
CMR substances in categories 1A or 1B which are not on the
candidate list, exceeding 0.1 percentage by mass: NO.
Biocide products were added to this construction product or it
has been treated with biocide products (this then concerns a
treated product as defined by the (EU) Ordinance on Biocide
Products No. 528/2012): NO.
2.6 Manufacture
The raw material for MT-100 OC is sourced from Bremen,
Germany and transported to Gresten, Austria via train. The
profile is manufactured through a cold-roll forming process of
steel sheets which also includes cutting to designated lengths
at the end of the line.
2.2 Application
The MT-100 OC is developed to be fixed on base materials like
concrete and steel frame structure to support the mechanical,
electrical, and piping services so that their loads are transferred
to the super structure of the building or facility. The product is
intended to be used under outdoor conditions for supporting:
- Pipes for the transport of fluids and gas
- Technical building equipment in general
- Components of fixed fire-fighting systems
- Electrical cable layouts 2.7 Environment and health during manufacturing
- Ventilating system layouts and equipment
Hilti ensures that the suppliers implement a quality
- Flooring
management system that meets the requirements of the ISO
- Other instrumentation
9001 or ISO/TS 16949 standards or higher. Quality must be
planned, ensured and documented using appropriate quality
2.3 Technical Data
tools, e.g. Statistical process control (SPC) or failure, mode and
The following data complies to the dimension drawing provided
effects analysis (FMEA). The production and quality control
in the Annexe A3 of ETA-21/0414.
according to the product specifications and approval
Constructional data specifications of the MT profile and its system components are
ensured by an in-house quality control by Hilti.
We expect the environmental management implemented by our
suppliers to meet at least the ISO14001 standard international
regulations on forbidden substances.
3 Environmental Product Declaration - HILTI AG - MT- System (Outdoor)
use involve weathering as well as mechanical loads.
The supplier for the MT-100 OC holds the following
certifications: 2.13 Extraordinary effects
- ISO 9001 Fire
- ISO 45001 The MT-100 OC is assessed in accordance with the European
- ISO 14001 Assessment Document EAD 280016-00-0602 for the following
performance in safety in case of fire (BWR2).
2.8 Product processing/Installation
Fire protection
The MT-100 OC is supplied as a ready to install modular
Name Value
support system element provided with an Instruction for Use
explaining the basic steps for installation. Reaction to fire Class A1
The MT-100 OC is either connected to a pre-positioned Pull-through resistance of channel back holes ETA
baseplate element that connects it to the building structure or is under fire exposure 23/0105
positioned directly to the building structure when delivered as a ETA
Bending characteristics under fire exposure
pre-assembled module. For fastening the connection point to 23/0105
the baseplate or other connection elements, a Hilti automated
impact wrench tool called SIW 6AT-A22 may be used to ensure
Water
anchoring or bolting at precise fastening torques. No special
The MT-100 OC is comprised of continuous hot-dip coated
environmental protection measures need to be taken while
steel. There are no environmental risks attributable to the
installing the MT profiles.
effects of water except the product's own corrosion impact.
2.9 Packaging
The MT-100 OC is delivered packed and strapped in bundles Mechanical destruction
as long goods. The product type can be either in 3 meter In the event of mechanical destruction of the MT-100 OC, the
lengths or 6 meter lengths. Same length types are bundled profile assembly has to be replaced with a new set for the
together in steel straps and delivered on wooden blocks that intended functional performance.
protect the ends of the bundles. Depending on the usage case
2.14 Re-use phase
and user request, the profile can be cut into various lengths as
The MT-100 OC cannot be re-used as a component for a
requested and bundled or preassembled in customized
modular support system, but the material can be recycled. All
conditions.
components of the described product can be returned and
Both the wooden blocks and steel straps cannot be re-used but
recycled into the material cycle.
can be recycled.
2.15 Disposal
2.10 Condition of use
The MT-100 OC is disassembled from a building in which it has
All supplied materials are protected in the installed condition
been installed by a series of unfastening processes. The
against external influences and designed for the service life of
interfaces with assembly components and with concrete or
the respective construction.
steel structures which have been originally fastened with a bolt
2.11 Environment and health during use and nut mechanism are untightened and separated back into
When used as designated, there is no impact on the individual product parts without change or deformation of the
environment or health. product material. These are fed into the recycling process in
accordance with the applicable disposal guidelines. The waste
2.12 Reference service life code for the profiles in accordance with the European Waste
The MT-100 OC has an assumed service life of 50 years in Index is 17 04 05 (iron and steel).
accordance with the BBSR table 'Service lives of Components
2.16 Further information
for life cycle assessment according to BNB'. The practical
service life can however be considerably longer and will Further information is available on the Hilti website:
depend on the specific installation situation and the product www.hilti.group
exposure scenario. The main factors influencing the period of
3. LCA: Calculation rules
Type of EPD: Cradle to factory gate with options. The following
3.1 Declared Unit information modules are defined as system boundaries in this
The declared product here is a mounting system from HILTI AG study:
with the designation I.-Girder MT-100 OC as a representative
product from the MT Outdoor portfolio. The declared unit refers
to 1 kg of mounting system. The packaging, related to 1 kg of Production stage (A1- A3):
mounting rail, is additionally included in the calculation with - A1, raw material extraction,
0.007 kg. The following table shows the data of the declared - A2, transport to the manufacturer,
unit. - A3, production.
Declared unit and mass reference
Name Value Unit
End of life (C1- C4):
Declared unit 1 kg
- C1, deconstruction/demolition,
Gross density 7850 kg/m3 - C2, transport,
Mass reference 14,8 kg/m - C3, waste treatment ,
- C4, disposal.
conversion factor 14,8
3.2 System boundary
4 Environmental Product Declaration - HILTI AG - MT- System (Outdoor)
Reuse, recovery and recycling potential (D). The cut-off criterion according to EN 15804+A2 is otherwise not
applied. All energy and mass inputs were taken into account.
In order to accurately capture the indicators and environmental 3.5 Background data
impacts of the declared unit, a total of 8 information modules The background data referred to in this study comes from
are considered. The information modules A1 to A3 describe the Sphera's LCA for Experts database.
material provision, the transport to the production site, as well
3.6 Data quality
as the production processes of the product itself.
For the preparation of the LCA, specific data from the Gersten
plant in Austria of HILTI AG from the year 2022 were collected.
The primary products are sourced from the European Union. The background data from the LCA for Experts database is
The transport is carried out by lorry and train. The following flow from 2023 and therefore highly relevant.
charts illustrate the underlying production process. The data quality is rated as adequate.
3.7 Period under review
The input and output flows used in this calculation come from
the annual average consumption from the year 2022.
Illustration 1: Information modules A1 to A3 of product 3.8 Geographic Representativeness
Land or region, in which the declared product system is
manufactured, used or handled at the end of the product´s
lifespan: Global
3.9 Allocation
The assembly system I.-Girder MT-100 OC as a representative
product of the MT Outdoor portfolio is produced in Gresten in
Illustration 2: Information modules A1 to A3 of packaging
Austria. The data for input and output flows are taken from the
year 2022, which corresponds to the annual average. The input
In the information modules C1 to C4, the deconstruction or
and output flows used in this calculation were measured directly
demolition from the building, the transport to waste disposal,
by the manufacturer for this production process and are shown
the waste treatment and disposal of the product are recorded.
in the following table. To calculate the net flows, the mass that
Furthermore, reuse, recovery and recycling potentials are
is generated as production waste in the production process and
reported in information module D.
is used as external steel scrap is subtracted from the total mass
of secondary material.
3.3 Estimates and assumptions
A steel coil with zinc content was used for the I.-Grider MT-100 3.10 Comparability
OC. The
Basically, a comparison or an evaluation of EPD data is only
transport of the lubricant was not taken into account, as
possible if all the data sets to be compared were created
themass fraction is small and the effect is estimated to be low
according to EN 15804 and the building context, respectively
the product-specific characteristics of performance, are taken
3.4 Cut-off criteria
into account. The database referred to in this study is LCA for
The transport for the lubricant was not taken into account as
Experts by Sphera.
the mass fraction is small. The lubricant itself was taken into
account in the production for transparency of production.
4. LCA: Scenarios and additional technical information
consumption for the tool is assumed to be 0.003 MJ for the
Characteristic product properties of biogenic carbon specified unit. The electricity consumption is calculated with a
The declared product does not contain any biogenic German electricity mix.
Carbon. In information module C3, the waste treatment (sorting and
Information on describing the biogenic Carbon Content at pressing) of the steel is calculated. med to be 0.003MJ for the
factury gate declared unit. The electricity consumption is calculated with a
German electricity mix
Name Value Unit
Name Value Unit
Biogenic carbon content in accompanying kg
packaging 0.0018 C Collected separately waste type waste type 1 kg
Recycling 1 kg
Note: 1 kg of biogenic carbon is equivalent to 44/12 kg of CO .
2
Reuse, recovery and/or recycling potentials (D), relevant
scenario information
In Module D, a recycling rate of 85% is assumed (world steel
End of life (C1-C4) association).
In information module C1, the demolition of the mounting Name Value Unit
system from the building is calculated. The demolition is carried Recycling 0,85 kg
out with an electric screwdriver. The electrical energy
5 Environmental Product Declaration - HILTI AG - MT- System (Outdoor)
5. LCA: Results
DESCRIPTION OF THE SYSTEM BOUNDARY (X = INCLUDED IN LCA; MND = MODULE OR INDICATOR NOT DECLARED; MNR
= MODULE NOT RELEVANT)
Benefits and
Construction loads beyond
Product stage Use stage End of life stage
process stage the system
boundaries
la ire ta m w a Ry lp p u s tro p s n a rT g n iru tc a fu n a M e h t m o rf tro p s n a rTe tis e h t o t e ta g y lb m e s s A e s U e c n a n e tn ia M ria p e R tn e m e c a lp e R tn e m h s ib ru fe R y g re n e la n o ita re p Oe s u re ta w la n o ita re p Oe s u n o itc u rts n o c -e Dn o itilo m e d tro p s n a rT g n is s e c o rp e ts a W la s o p s iD -e s u e R-y re v o c e R-g n ilc y c e Rla itn e to p
A1 A2 A3 A4 A5 B1 B2 B3 B4 B5 B6 B7 C1 C2 C3 C4 D
X X X MND MND MND MND MNR MNR MNR MND MND X X X X X
RESULTS OF THE LCA - ENVIRONMENTAL IMPACT according to EN 15804+A2: 1 kg I.Girder MT-100 OC
Parameter Unit A1-A3 C1 C2 C3 C4 D
Global Warming Potential total (GWP-total) kg CO 2 eq 2.85E+00 7.28E-04 4.42E-03 1.69E-02 0 -1.89E+00
Global Warming Potential fossil fuels (GWP-fossil) kg CO 2 eq 2.85E+00 7.28E-04 4.39E-03 1.69E-02 0 -1.89E+00
Global Warming Potential biogenic (GWP-biogenic) kg CO 2 eq 2.92E-03 1.58E-07 0 4.11E-06 0 -1.02E-03
Global Warming Potential luluc (GWP-luluc) kg CO 2 eq 1.32E-03 1.06E-07 2.61E-05 2.12E-06 0 -6.72E-04
Depletion potential of the stratospheric ozone layer (ODP) kg CFC11 eq 2.14E-12 4.29E-17 7.63E-16 1.58E-10 0 -1.42E-12
Acidification potential of land and water (AP) mol H+ eq 6.56E-03 8.57E-07 1.69E-05 9.99E-05 0 -4.14E-03
Eutrophication potential aquatic freshwater (EP-freshwater) kg P eq 2.84E-06 7.24E-11 1.02E-08 3.05E-07 0 -1.44E-06
Eutrophication potential aquatic marine (EP-marine) kg N eq 1.65E-03 2.85E-07 8.07E-06 4.53E-05 0 -1.06E-03
Eutrophication potential terrestrial (EP-terrestrial) mol N eq 1.8E-02 3.1E-06 9.02E-05 4.92E-04 0 -1.14E-02
Formation potential of tropospheric ozone photochemical oxidants kg NMVOC
5.49E-03 7.87E-07 1.53E-05 1.45E-04 0 -3.5E-03
(POCP) eq
Abiotic depletion potential for non fossil resources (ADPE) kg Sb eq 1.14E-07 3.01E-12 3.09E-10 3.49E-09 0 -7.25E-08
Abiotic depletion potential for fossil resources (ADPF) MJ 3.78E+01 1.07E-02 5.92E-02 2.29E-01 0 -1.68E+01
m3 world eq
Water use (WDP) 3.42E-02 4.08E-06 2.27E-05 4.76E-04 0 -2.2E-02
deprived
RESULTS OF THE LCA - INDICATORS TO DESCRIBE RESOURCE USE according to EN 15804+A2: 1 kg I.Girder MT-100 OC
Parameter Unit A1-A3 C1 C2 C3 C4 D
Renewable primary energy as energy carrier (PERE) MJ 1.55E+00 4.08E-05 3.83E-03 1.12E-03 0 -9.97E-01
Renewable primary energy resources as material utilization
MJ 8E-02 0 0 0 0 0
(PERM)
Total use of renewable primary energy resources (PERT) MJ 1.63E+00 4.08E-05 3.83E-03 1.12E-03 0 -9.97E-01
Non renewable primary energy as energy carrier (PENRE) MJ 3.81E+01 1.07E-02 5.92E-02 2.29E-01 0 -1.69E+01
Non renewable primary energy as material utilization (PENRM) MJ 0 0 0 0 0 0
Total use of non renewable primary energy resources (PENRT) MJ 3.81E+01 1.07E-02 5.92E-02 2.29E-01 0 -1.69E+01
Use of secondary material (SM) kg 0 0 0 0 0 0
Use of renewable secondary fuels (RSF) MJ 0 0 0 0 0 0
Use of non renewable secondary fuels (NRSF) MJ 0 0 0 0 0 0
Use of net fresh water (FW) m3 1.67E-03 1.61E-06 3.48E-06 2.52E-05 0 -9.95E-04
RESULTS OF THE LCA – WASTE CATEGORIES AND OUTPUT FLOWS according to EN 15804+A2:
1 kg I.Girder MT-100 OC
Parameter Unit A1-A3 C1 C2 C3 C4 D
Hazardous waste disposed (HWD) kg 5.16E-10 5.45E-13 1.59E-13 5.05E-12 0 4.42E-11
Non hazardous waste disposed (NHWD) kg 3.1E-02 2.81E-06 8.63E-06 2.6E-05 0 -2.3E-02
Radioactive waste disposed (RWD) kg 1.87E-04 9.32E-07 6.19E-08 8.63E-06 0 -9.96E-05
Components for re-use (CRU) kg 0 0 0 0 0 0
Materials for recycling (MFR) kg 6.43E-03 0 0 8.5E-01 0 0
Materials for energy recovery (MER) kg 0 0 0 0 0 0
Exported electrical energy (EEE) MJ 0 0 0 0 0 0
Exported thermal energy (EET) MJ 0 0 0 0 0 0
RESULTS OF THE LCA – additional impact categories according to EN 15804+A2-optional:
1 kg I.Girder MT-100 OC
Parameter Unit A1-A3 C1 C2 C3 C4 D
Disease
Incidence of disease due to PM emissions (PM) ND ND ND ND ND ND
incidence
6 Environmental Product Declaration - HILTI AG - MT- System (Outdoor)
Human exposure efficiency relative to U235 (IR) kBq U235 eq ND ND ND ND ND ND
Comparative toxic unit for ecosystems (ETP-fw) CTUe ND ND ND ND ND ND
Comparative toxic unit for humans (carcinogenic) (HTP-c) CTUh ND ND ND ND ND ND
Comparative toxic unit for humans (noncarcinogenic) (HTP-nc) CTUh ND ND ND ND ND ND
Soil quality index (SQP) SQP ND ND ND ND ND ND
Disclaimer 1 – for the indicator 'Potential Human exposure efficiency relative to U235'. This impact category deals mainly with the
eventual impact of low-dose ionizing radiation on human health of the nuclear fuel cycle. It does not consider effects due to possible
nuclear accidents, occupational exposure or radioactive waste disposal in underground facilities. Potential ionizing radiation from the
soil, from radon and some construction materials is also not measured by this indicator.
Disclaimer 2 – for the indicators 'abiotic depletion potential for non-fossil resources', 'abiotic depletion potential for fossil resources',
'water (user) deprivation potential, deprivation-weighted water consumption', 'potential comparative toxic unit for ecosystems', 'potential
comparative toxic unit for humans – cancerogenic', 'Potential comparative toxic unit for humans - not cancerogenic', 'potential soil
quality index'. The results of this environmental impact indicator shall be used with care as the uncertainties on these results are high
as there is limited experience with the indicator.
6. LCA: Interpretation
The dominance analysis shows that the main causes of the The mounting system itself accounts for 99% of the total global
environmental impacts and indicators can be found in the warming potential in the A1 information module. Approximately
information module A1. This shows the total global warming 1% is accounted for by the steel strap.
potential for material supply with approx. 50% and approx. 8%
in production, based on all information modules.
Illustration: Dominance analysis A1- A3
Looking at the material supply of the assembly system and the
packaging in the de-tail, it becomes clear which raw materials
contribute decisively to the respective environmental impacts Illustration: Dominance analysis A1
and indicators.
7. Requisite evidence
The MT-100 OC may be used to constitute a supporting system systems and cable ladder systems. Therefore, requisite
to carry the load of cable trays and ladders but is not within evidence pertaining to this standard shall not be given for this
scope of the DIN EN 61537 which is specific to cable tray product.
8. References
Standards EN 61537
DIN EN 61537 VDE 0639:2007-09 ,
EN 10346:2015 Cable management
Continuously hot-dip coated steel flat products for cold fo ming - Cable tray systems and cable ladder systems
Technical delivery conditions (IEC 61537:2006); German version EN 61537:2007
EN 15804 ISO 9001:2015
EN 15804:2012+A1 2013, Sustainability of construction works Quality management system
— Environmental Product Declarations — Core rules for the
product category of construction products. ISO 14001:2015
Environmental Management System
EN 15804
EN 15804:2012+A2:2019+AC:2021, Sustainability of ISO 14025
construction works — Environmental Product Declarations — EN ISO 14025:2011, Environmental labels and declarations —
Core rules for the product category of construction products. Type III environmental declarations — Principles and
procedures
7 Environmental Product Declaration - HILTI AG - MT- System (Outdoor)
e.V.,2021 www.ibu-epd.de
ISO 15686
Buildings and constructed assets PCR Part A
Institut Bauen und Umwelt e.V, Berlin (pub.): Product Category
ISO 45001:2018 Rules for Construction Products from the range of
Occupational health and safety system Environmental Product Declarations for Institut Bauen und
Umwelt (IBU), Part A: Calculation Rules for the Life Cycle
Further references Assessment and Requirements on the Project Report according
to EN 15804+A2:2019, 202108
Candidate List of substances of very high concern for
Authorisation PCR Part B
European Chemicals Agency (ECHA), in accordance with Connection, assembly and installation systems,.10.2022
Article 50(10) of the REACH regulation
Regulation (EU) No. 305/2011 (CPR)
European Technical Approval ETA-21/0414 Hilti Installation Regulation (EU) No 305/2011 of the European Parliament
channels of MT system andof the Council of 9 March 2011 laying down
assessed based on EAD 280016-00-0602 'Products for harmonisedconditions for the marketing of construction
installation systems for supporting technical building equipment' products andrepealing Council Directive 89/106/EEC Text with
EEArelevance
European Technical Approval ETA-23/0105
Sphera
LCA for Experts: Ganzheitliche Bilanzierung
European Waste code Leinfelden-Echterdingen; Sphera Solution GmbH (Hrsg.)
in accordance with the European Waste Catalogue (EWC) http://www.gabi-software.com/deutsch/index/
(EWC 2014/955/EU) Commission Decision amending Decision
2000/532/EC on the list of waste pursuant to Directive World steel association
2008/98/EC of the European Parliament and of the Council https://www.worldsteel.org/steel-topics/raw-materials/
IBU 2021
General Instructions for the EPD programme of Institut Bauen
und Umwelt e.V. Version 2.0, Berlin: Institut Bauen und Umwelt
8 Environmental Product Declaration - HILTI AG - MT- System (Outdoor)
Publisher
Institut Bauen und Umwelt e.V. +49 (0)30 3087748- 0
Hegelplatz 1 info@ibu-epd.com
10117 Berlin www.ibu-epd.com
Germany
Programme holder
Institut Bauen und Umwelt e.V. +49 (0)30 3087748- 0
Hegelplatz 1 info@ibu-epd.com
10117 Berlin www.ibu-epd.com
Germany
Author of the Life Cycle Assessment
FIT-Umwelttechnik GmbH 05362 72 69 474
Westerstr. 13 bertram@fit-umwelttechnik.de
38442 Wolfsburg www.fit-umwelttechnik.com
Germany
Owner of the Declaration
Hilti Aktiengesellschaft +423 234 2111
Feldkircher Strasse 100 HAGHSE@hilti.com
9494 Schaan www.hilti.com
Liechtenstein
9 Environmental Product Declaration - HILTI AG - MT- System (Outdoor)
