ENVIRONMENTAL PRODUCT DECLARATION
as per ISO 14025 and EN 15804+A2
Owner of the Declaration Unilin B.V. Division Panels
Publisher Institut Bauen und Umwelt e.V. (IBU)
Programme holder Institut Bauen und Umwelt e.V. (IBU)
Declaration number EPD-UNI-20230378-IBJ1-EN
Issue date 31.10.2023
Valid to 30.10.2028
Unilin Medium Density Fiberboard
Unilin B.V. Division Panels
www.ibu-epd.com | https://epd-online.com
1. General Information
Unilin B.V. Division Panels Unilin Medium Density Fiberboard
Programme holder Owner of the declaration
IBU – Institut Bauen und Umwelt e.V. Unilin B.V. Division Panels
Hegelplatz 1 Ooigemstraat 3
10117 Berlin 8710 Wielsbeke
Germany Belgium
Declaration number Declared product / declared unit
EPD-UNI-20230378-IBJ1-EN 1 m³ Unilin medium density fiberboard (637 kg/m³)
This declaration is based on the product category rules: Scope:
Wood-based panels, 01.08.2021 The scope of this EPD extends to Unilin's entire raw medium density
(PCR checked and approved by the SVR) fiberboard (MDF) range. The values declared refer to the sales-weighted
average product. These are produced in following manufacturing sites:
• Bazeilles, France
Issue date
• Vielsalm, Belgium
31.10.2023
The owner of the declaration shall be liable for the underlying information
and evidence; the IBU shall not be liable with respect to manufacturer
Valid to information, life cycle assessment data and evidences.
30.10.2028
The EPD was created according to the specifications of EN 15804+A2. In
the following, the standard will be simplified as EN 15804.
Verification
The standard EN 15804 serves as the core PCR
Independent verification of the declaration and data according to ISO
14025:2011
internally X externally
Dipl.-Ing. Hans Peters
(Chairman of Institut Bauen und Umwelt e.V.)
Florian Pronold Mr Olivier Muller,
(Managing Director Institut Bauen und Umwelt e.V.) (Independent verifier)
1 Environmental Product Declaration - Unilin B.V. Division Panels - Unilin Medium Density Fiberboard
2. Product
• MDF.H : General purpose boards for use in humid
2.1 Product description/Product definition conditions
A medium density fiberboard is a versatile engineered wood • MDF.LA : Load-bearing boards for use in dry conditions
product designed for various applications. It is generated by • MDF.HLS : Load-bearing boards for use in humid
compressing wood fibers and glue under high pressure and conditions
temperature, resulting in a smooth, homogeneous panel with • L-MDF : Light MDF boards for use in dry conditions
excellent strength and dimensional stability. • L-MDF.H : Light MDF boards for use in humid conditions
• UL1-MDF : Ultra-light MDF boards for use in dry
For the placing on the market of the product in the European conditions
Union/European Free Trade Association (EU/EFTA) (with the • UL2-MDF : Ultra-light MDF boards for use in dry
exception of Switzerland) Regulation (EU) No. 305/2011 (CPR) conditions
applies. The product needs a declaration of performance • MDF.RWH : For use in rigid underlays in roofs and walls
according to:
2.3 Technical Data
• EN 13986:2004+A1:2015, Wood-based panels for use
Technical characteristics vary by product variant and thickness.
in construction – Characteristics, valuation of conformity
More detailed product-specific data, technical data sheets and
and marking
the CE declaration of performance are available on
• EN 622-5:2010, Fibreboards - Specifications - Part 5:
www.unilinpanels.com.
Requirements for dry process boards (MDF)
Constructional data
For its application and use the respective national provisions The table below summarizes the technical performance of
apply. Unilin's raw MDF range for some parameters. The values below
apply to the product range. More information on these ranges
The results in this EPD refer to the environmental impact of a and additional parameters is available at the product's
raw MDF board with a sales-weighted average. The "Declaration Of Performace" on www.unilinpanels.com. Specific
composition of this product was obtained by averaging Unilin's properties of the declared sales-weighted product are available
entire MDF portfolio using the annual sales volumes as in 3.10.
weighting factor. The declared impact is thus representative for
Name Value Unit
the following commercial references (available in thicknesses
Gross Density (EN
6 - 40 mm): 350 - 750 kg/m³
323)
• Fibrabel (Black) (LF+/NAF)
Bending strength
• Fibrabel Featherlight/Exteremlight/Ultralight (LF+/NAF) 25 - 30 N/mm²
(EN 310)
• Fibrabel FR (Uncoloured) (Class C/XP/Wheelmark)
E-modulus (EN 310) 560 - 2700 N/mm²
• Fibrabel MR (Uncoloured) (FR) (NAF/LF+) (MR50)
• Fibralux FR (Black/Uncoloured) (Class Swelling 24h (EN
8 - 14 %
C/XP/Wheelmark)) 317))
• Fibralux MR (FR) (Black/Grey/Uncoloured) (NAF/LF+) Tensile strength (EN
0.15 - 0.75 N/mm²
(MR50) 319)
• Fibralux (Plus/Ultralight) (LF+/NAF) E1(*); E0.5 (**); CARB/TSCA Title
Formaldehyde
• Fibralux Pro (P/MR) (Uncoloured) (LF+/NAF/Svanen) VI (***); F****(****)
• RWH (LF+) (TG)
Different formaldehyde emission standards are available :
• Fibrofit (Ultralight/FI) (Charcoal) (LF/LF+)
(*) E1 - According to EN 13986+A1:2015 :
• Fibrofit MR (Uncoloured) (LF/LF+)
• Fibromax (FI) (LF/LF+) • a limit value of 0.1 ppm may not be exceeded by EN
• Fibromax MR (Uncoloured) (LF/LF+) 717-1 emission chamber method OR
• Fibromax Pro (MR/FI) (LF/LF+)(Uncoloured) • a limit value of 8 mg HCHO/100 g according to ISO
12460-5
The values for specific commercial references can vary from
the declared ones. Please contact Unilin's sales team or (**) E0.5 - According to the ChemVerbotsV :
info.panels@unilin.com for more information.
• a limit value of 0.1 ppm according to EN 16516 OR
• a limit value of 0.05 ppm according to EN 717-1
2.2 Application
Unilin's MDF boards are highly versatile and used in both
(***) CARB 2/TSCA Title VI - According to California Air
structural and non-structural applications. The surface variety
Resources Board & the US Toxic Substances Control Act
accommodates the use of a versatile range of finishes and
(TSCA Title VI) :
coatings, making the material easy to use in many different
designs and applications. • a limit value of 0.13 ppm (thickness < 8 mm) according
to ASTM E1333 or ASTM D6007
The product is predominantly used with a coated surface. • a limit value of 0.11 ppm (thickness ≥ 8 mm) according
Fiberboards are typically used in furniture as counters, to ASTM E1333 or ASTM D6007
worktops, displays, wall coverings. MDF boards are also (****) F**** - According to Japanese standard JIS A 5908
suitable for manufacturing doors and frames (coated, foiled, • a limit value of 0.3 mg/L according to JIS A 1460
painted) and can be milled due to their homogeneous structure. desiccator
Performance data are consistent with the product's declaration
Unilin Fiberboards can be used in a variety of applications, of performance with respect to its essential characteristics
classified according EN 622-5:2010 : according to:
• MDF : General purpose boards for use in dry conditions
2 Environmental Product Declaration - Unilin B.V. Division Panels - Unilin Medium Density Fiberboard
constantly improve environmental performance. The Bazeilles
• EN 13986:2004+A1:2015, Wood-based panels for use
plant is ISO 9001 and ISO 50001 certified. The Vielsalm site is
in construction – Characteristics, valuation of conformity
certified under ISO 9001, ISO 14001 and ISO 45001.
and marking
• EN 622-5:2010, Fibreboards - Specifications - Part 5:
The implementation of Unilin's One Home Sustainability
Requirements for dry process boards (MDF)
Strategy and its Zero Harm Safety Policy have further set clear
2.4 Delivery status targets to among others reduce the carbon footprint of its
Unilin offers its fiberboard range in a variety of sizes, the most production activities, enhance the overall resource efficiency
common ones being: and improve the safety and well-being at its production sites.
• 1220 x 2440 mm 2.8 Product processing/Installation
• 1220 x 3050 mm The Unilin MDF board can be processed (e.g. sawing, milling,
• 1310 x 3050 mm drilling) using common utility tools and machinery. It is advised
• 2070 x 2800 mm to wear a dust mask when tools are used without dust
• 2070 x 4100 mm extraction. More specific processing and health information is
• 2200 x 3660 mm available at www.unilinpanels.com.
These are available in thicknesses ranging from 6 to 40 mm. 2.9 Packaging
Other dimensions can be produced on request. Please contact Packaging is used to protect the product from damage during
info.panels@unilin.com. transport. Wood-based pallets, cardboard, paper labels, stretch
foil and PET/steel-based packaging straps are used as
2.5 Base materials/Ancillary materials
packaging materials.
The table below details the sales-weighted average
composition for 1 m³ of the Unilin MDF board. This product has 2.10 Condition of use
a density of 637 kg/m³ and and consists of fresh wood, glue, The product's composition remains unchanged during its use
additives and moisture. The glue is either based on a and is therefore the same as stated in section 2.5. The glue and
(melamine) urea formaldehyde (M(UF)) mixture or pMDI additives are permanently bonded to the wood through an
(polymeric form of 4,4'-Methylene diphenyl diisocyanate). The irreversible curing process.
additives added depend heavily on the specific commercial
reference (e.g. wax emulsion, fire retardant based on inorganic 2.11 Environment and health during use
salts). Based on current knowledge, using the Unilin fiberboard as
Name Value Unit intended poses no risks to health, water, air or soil. Small
amounts of natural wood constituents could potentially be
Fresh wood 81 %
released, but aside from negligible amounts of formaldehyde,
Glue 11 %
no harmful emissions have been detected.
Additives 2 %
2.12 Reference service life
Moisture 6 %
The reference service life (RSL) of the product depends
The fresh wood is 100 % recovered wood, predominantly
significantly on its field of use. Please contact Unilin's sales
sourced from sustainable forest management activities and
team or info.panels@unilin.com for more specific information
sawmills (residues & co-products), and mainly consists of
on the product's lifespan in a given set of conditions.
spruce, beech and birch.
The fiberboard's RSL can vary from 10 to 40 years depending
The composition of specific commercial references can differ
on its area of application; according to the BBSR table "BNB
from the values depicted above and can be obtained by
Nutzungsdauern von Bauteilen (2017)".
reaching out to info.panels@unilin.com.
2.13 Extraordinary effects
Unilin's fiberboard range contains no Substances of Very High Fire
Concern (SVHCs) or Category 1A or 1B CMR-substances (as The fire resistance of the Unilin MDF board depends heavily on
defined by ECHA) above 0.1 % by weight: No its chemical composition (i.e. presence of fire retardants). The
The fiberboards further contain no biocides as defined under products have the following fire behaviour (according to
the EU Biocidal Products Ordinance No. 528/2012 nor are the EN13501-1):
boards treated with such substances.
CE AVCP Class 4 :
2.6 Manufacture
• Standard/Moisture Resistant fiberboards (excl. fire
1. Round wood is collected to produce the fiberboards.
retardant): D-s2,d0 (≥ 9mm & Bulk density > 600 kg/m³)
2. The bark is removed from the round wood logs.
3. The logs are chopped to wood chips.
CE AVCP Class 1 :
4. The wood chips are defibrated under high pressure in a
refiner. • Fibrabel FR: B-s2,d0 (10-15 mm), B-s1,d0 (15-30 mm)
5. The board is produced by introducing the fibermat into a • Fibrabel FR XP: C-s2,d0 (12-25 mm)
press, which compresses it under higher pressure and • Fibrabel MR FR NAF: B-s1,d0 (12 - 25 mm)
temperature. • Fibralux FR: B-s2,d0 (6-12 mm), B-s1,d0 (12-30 mm)
6. The board is sanded, cut into panels and finished • Fibralux FR Black: B-s2,d0 (9-15.9 mm), B-s1,d0 (16-19
depending on the intended application. mm)
• Fibralux FR (UC) XP: C-s2,d0 (6-25 mm)
2.7 Environment and health during manufacturing • Fibralux FR MR NAF: B-s1-d0 (6-30 mm)
Unilin's plant management policy is fully integrated in the daily
operation and governance of its production plants. The aim is to Fire reaction classes are part of the CE Declaration of
adhere to legal requirements, minimize negative environmental Performance available on Unilin Panels website
effects on its neighbors, co-workers and surroundings, and www.unilinpanels.com.
3 Environmental Product Declaration - Unilin B.V. Division Panels - Unilin Medium Density Fiberboard
Energy Recovery
Water In line with the cascading use of wood-based products, the
The Unilin fiberboard does not contain substances that may reuse of the end-of-life MDF should be prioritized. However, if
potentially contaminate water through leaching. However, it is this is not feasible, the board can be used as a secondary fuel
important, to ensure that the product is not subjected to in approved energy power plants. Its relatively high calorific
continuous exposure to moisture. Prolonged contact with water value enables power plants to effectively produce renewable
may result in the degradation of the product. heat and electricity.
Mechanical destruction 2.15 Disposal
When subjected to mechanical stress, the product displays a Jobsite and post-consumer MDF-waste (e.g. from demolition
tendency towards brittleness. This could result in the formation projects) should be reused/recycled where possible, in line with
of sharp broken edges, which may pose a risk of injury. the cascade principle. Should this not be possible, the waste
must be utilized for energy recovery as opposed to being
2.14 Re-use phase landfilled (in accordance with EWC waste codes
Reuse 170201/030105).
When a building or furniture has reached its end-of-life phase,
the Unilin fiberboard can easily be abstracted and collected if Waste from packaging materials, which protect the product
selective dismantling/sorting takes place. After collection, the from damage during transport, can be reused and recycled if
end-of-life fiberboard can be reused for the same (or different) sorted correctly.
purpose if possible.
2.16 Further information
Please contact Unilin's sales team or reach out to
info.panels@unilin.com for additional information.
3. LCA: Calculation rules
3.1 Declared Unit C2: Transport to Waste Processing
The declared information and values refer to 1 m³ of Unilin MDF This life cycle stage describes the impact of the end-of-life
board with a sales-weighted average composition and density product's transport from the demolition site to the waste
of 637 kg/m³. processing facility. A representative distance of 50 km is
Declared unit and mass reference assumed.
Name Value Unit
C3: Waste Processing
Declared unit 1 m3 Processing of the post-consumer MDF waste involves
Gross density 637 kg/m3 (preliminary) sorting and shredding of the material. The
fiberboard is repurposed as a secondary fuel and undergoes
The composition of the Unilin fiberboard, for which values are
energy recovery in module D. The material and its inherent
declared in this EPD, was obtained by averaging Unilin's entire
properties (e.g. biogenic carbon and primary energy content)
MDF portfolio based on the annual sales volumes. The product
are thus exported from the system in C3.
is manufactured at the Bazeilles and Vielsalm plants, which are
both in the scope of this declaration.
C4: Waste Disposal
3.2 System boundary This module describes the loads and emissions attributed to
the disposal of the product after waste processing. As the end-
This is a cradle-to-gate EPD with options, including the
of-life product leaves the system in C3 as a secondary fuel, no
following life cycle phases A1 - A3, C1 - C4 and D. The
environmental impact is declared in C4.
following processes have been considered for each of the
modules:
D: Loads and Benefits beyond the System Boundaries
Module D describes the loads and benefits related to the use of
A1 - A3: Product Stage
the end-of-life MDF as a secondary fuel. This involves the
The production stage encompasses the extraction of raw
energy recovery of post-consumer fiberboard waste, where it
materials (i.e. wood, glue, additives), their transportation to the
replaces a European-averaged mix of electricity and heat.
production plants, and the subsequent manufacturing of the
product. The required energy for production, ancillary materials,
The system boundary between subsequent systems is defined
and production emissions are included. Energy and material
in accordance with EN 15804+A2, i.e. when the material
input/output data were obtained from Unilin's fiberboard
reaches its end-of-waste state. End-of-life fiberboard reaches
factories (Bazeilles and Vielsalm) as well as Unilin's glue
its end-of-waste state after a sorting and shredding step, as
factory.
inventoried in C3. The material leaves the current system at
module C3 and enters a subsequent system as a secondary
A large share of the used thermal energy is derived from
fuel.
renewable sources, such as internal and external woody waste
streams. Any remaining energy needs are met through the local
3.3 Estimates and assumptions
grid in Belgium or France.
Specific, primary data have been used to the highest extent
possible. In case of absence, estimates and assumptions were
C1: Deconstruction/Demolition stage
made to model reality as closely as possible. These
It is assumed that the end-of-life fiberboard is manually
assumptions are based on publicly available data and literature.
dismantled from the building/furniture. The efforts involved in
Generic dataset from the EcoInvent 3.8. database have been
this process are considered negligible, leading to the absence
used to model the impact of some raw materials and process-
of a declared environmental impact arising from the dismantling
related parameters for which specific data was lacking.
of the product.
4 Environmental Product Declaration - Unilin B.V. Division Panels - Unilin Medium Density Fiberboard
End-of-life fiberboard leaves the product system in C3 as a The technological, geographical, and time-related
secondary fuel, for which the benefits and loads are inventoried representativeness of background data (e.g. from EcoInvent)
in module D. Here it is assumed that the secondary fuel was verified, as stated in EN15804+A2.
substitutes electricity and heat in accordance with an average
mix available on the European grid. 3.7 Period under review
Primary data, needed to calculate the LCA of the system under
3.4 Cut-off criteria study, was collected for the year 2020 from the Bazeilles,
All in- and outputs to the system under study have been Vielsalm and Unilin's glue production facility.
included in the LCA. Primary data was used to the highest
extent possible. If primary data was lacking, secondary data 3.8 Geographic Representativeness
from EcoInvent was resorted to. Conservative assumptions Land or region, in which the declared product system is
were made using average or generic data in case of data gaps. manufactured, used or handled at the end of the product´s
These assumptions are based on publicly available (literature lifespan: Western Europe
reported) data. As such, all processes, materials, or emissions
expected to have a significant contribution to the environmental
3.9 Allocation
impact of the system under study were considered in the LCA.
In line with EN 15804+A2 and EN 16485, the biogenic carbon
The total sum of omitted flows can therefore be deemed as
and primary energy content of the wood have been balanced
significantly below the 5 % threshold of the system's energy
over the product's entire life cycle (A1 - C4) based on its
and mass input, as stated in the EN 15804+A2.
inherent material characteristics and underlying physical flows.
3.5 Background data Fresh wood inventories were taken from EcoIvent 3.8. Here, it
The relevant background data was either taken from the was made sure that the biogenic carbon and energy content
EcoInvent 3.8. database or peer-reviewed literature sources. reflect the physical relationships of the different wood-based
Measures were taken to ensure that the used secondary data materials.
was no more than 10 years old. These data types allowed to
map the background system in the LCA of the product under The system boundary (and subsequent allocation) relating to
study. the flow of the end-of-life product are as described in section
3.2.
3.6 Data quality
3.10 Comparability
Data collection and necessary calculations were done in line
with ISO 14044. Primary data was directly gathered from the Basically, a comparison or an evaluation of EPD data is only
designated person at Unilin's fiberboard and glue plants. It was possible if all the data sets to be compared were created
ensured that the collected data accurately represented reality, according to EN 15804 and the building context, respectively
so it can be assumed that the used primary data is of high the product-specific characteristics of performance, are taken
quality. into account. Background data was used from the EcoInvent
3.8. database.
4. LCA: Scenarios and additional technical information
Name Value Unit
Characteristic product properties of biogenic carbon
Wood-based pallet 1.06 kg/m³
The values declared below describe the amount of biogenic
Cardboard 0.39 kg/m³
carbon and stored biogenic CO in the building product under
2
Paper 0.039 kg/m³
study when it leaves the factory gate. These relate to 1 m³ of
Unilin MDF board, with a sales-weighted average composition. Stretch foil 0.087 kg/m³
PET straps 0.0076 kg/m³
Biogenic carbon content at factory gate
Steel-based straps 0.00044 kg/m³
The carbon uptake of the packaging materials is not included
below as their end-of-life impact is not declared in module A5. Information on the reference lifetime can be found in section
Name Value Unit 2.12. Please contact Unilin's sales team or
info.panels@unilin.com for more information.
Biogenic carbon content in product 253.3 kg C/m³
Stored carbon dioxide in product 928.7 kg CO2 eq./m³ End-of-life (C1-C4)
The following table provides the parameters required to model
Note: 1 kg biogenic carbon is equivalent to 44/12 kg CO .
2 the end-of-life of the product under study. Since the product is
not intended for extended outdoor use, it is assumed that its
moisture content remains consistent with its state at the factory
The following technical information is a basis for the declared
gate. The end-of-life product reaches its end-of-waste state
modules or can be used for developing specific scenarios in the
after (preliminary) sorting and shredding. The losses during the
context of a building assessment if modules are not declared
sorting and shredding are assumed to have a negligible impact
(MND).
and are thus discarded. The material leaves the system as a
Installation into the building (A5) secondary fuel (energy recovery).
The end-of-life impact of the used packaging materials is not
declared. However, its impact can be modelled based on the Name Value Unit
data given below for the sales-weighted average product.
Collected separately waste type waste type 637 kg
Secondary fuel (output at C3) 637 kg/m³
Reuse, recovery and/or recycling potentials (D)
In module D, the loads and benefits of exporting the secondary
fuel from the system under study are inventoried. The moisture
5 Environmental Product Declaration - Unilin B.V. Division Panels - Unilin Medium Density Fiberboard
content of this fuel is assumed to remain at a total of 6 %. This % as electricity. The generated energy carriers are assumed to
value may vary significantly based on the storage conditions substitute heat and electricity in accordance with the average
prior to its intended use. mix available on the European grid.
Name Value Unit
The recovery potential is modelled based on the net output flow
Net output flow of secondary fuel 608 kg/m³
of secondary fuel. It is assumed that a biomass power plant
Energy Efficiency Biomass plant 85 %
located in the EU recovers the secondary fuel's energy, with 55
% of the energy being recovered as heat and the remaining 30
6 Environmental Product Declaration - Unilin B.V. Division Panels - Unilin Medium Density Fiberboard
5. LCA: Results
The values declared below refer to 1 m³ of Unilin MDF board with a sales-weighted average composition and density of 637 kg/m³.
Table "Description of the system boundary" summarizes the scope of the system under study from a life cycle point of view. Declared
modules are indicated with an "X", non-declared modules are indicated with "MND". "MNR" refers to modules which are deemed as not
relevant.
DESCRIPTION OF THE SYSTEM BOUNDARY (X = INCLUDED IN LCA; MND = MODULE OR INDICATOR NOT DECLARED; MNR
= MODULE NOT RELEVANT)
Benefits and
Construction loads beyond
Product stage Use stage End of life stage
process stage the system
boundaries
la ire ta m w a Ry lp p u s tro p s n a rT g n iru tc a fu n a M e h t m o rf tro p s n a rTe tis e h t o t e ta g y lb m e s s A e s U e c n a n e tn ia M ria p e R tn e m e c a lp e R tn e m h s ib ru fe R y g re n e la n o ita re p Oe s u re ta w la n o ita re p Oe s u n o itc u rts n o c -e Dn o itilo m e d tro p s n a rT g n is s e c o rp e ts a W la s o p s iD -e s u e R-y re v o c e R-g n ilc y c e Rla itn e to p
A1 A2 A3 A4 A5 B1 B2 B3 B4 B5 B6 B7 C1 C2 C3 C4 D
X X X MND MND MND MND MNR MNR MNR MND MND X X X X X
RESULTS OF THE LCA - ENVIRONMENTAL IMPACT according to EN 15804+A2: 1 m³ Unilin MDF Board
Parameter Unit A1-A3 C1 C2 C3 C4 D
Global Warming Potential total (GWP-total) kg CO 2 eq -7.65E+02 0 2.75E+00 9.4E+02 0 -5.63E+02
Global Warming Potential fossil fuels (GWP-fossil) kg CO 2 eq 1.62E+02 0 2.75E+00 1.07E+01 0 -5.61E+02
Global Warming Potential biogenic (GWP-biogenic) kg CO 2 eq -9.28E+02 0 8.91E-04 9.29E+02 0 -1.11E+00
Global Warming Potential luluc (GWP-luluc) kg CO 2 eq 1.17E+00 0 1.06E-03 1.46E-02 0 -8.46E-01
Depletion potential of the stratospheric ozone layer (ODP) kg CFC11 eq 3.16E-05 0 6.91E-07 1.54E-06 0 -7.93E-05
Acidification potential of land and water (AP) mol H+ eq 1.2E+00 0 8.82E-03 6.05E-02 0 -7.78E-01
Eutrophication potential aquatic freshwater (EP-freshwater) kg P eq 1.24E-02 0 1.98E-05 5.9E-04 0 -3.71E-02
Eutrophication potential aquatic marine (EP-marine) kg N eq 4.21E-01 0 1.94E-03 1.54E-02 0 3.8E-01
Eutrophication potential terrestrial (EP-terrestrial) mol N eq 3.96E+00 0 2.16E-02 1.72E-01 0 4.12E+00
Formation potential of tropospheric ozone photochemical oxidants kg NMVOC
1.6E+00 0 8.5E-03 4.88E-02 0 7.43E-01
(POCP) eq
Abiotic depletion potential for non fossil resources (ADPE) kg Sb eq 2.07E-03 0 6.84E-06 3.58E-05 0 -1.84E-04
Abiotic depletion potential for fossil resources (ADPF) MJ 5.82E+03 0 4.51E+01 1.95E+02 0 -1.46E+04
m3 world eq
Water use (WDP) 2.3E+02 0 1.52E-01 5.41E-01 0 -7.99E+01
deprived
RESULTS OF THE LCA - INDICATORS TO DESCRIBE RESOURCE USE according to EN 15804+A2: 1 m³ Unilin MDF Board
Parameter Unit A1-A3 C1 C2 C3 C4 D
Renewable primary energy as energy carrier (PERE) MJ 4.71E+03 0 5.73E-01 9.69E+03 0 -1.2E+03
Renewable primary energy resources as material utilization
MJ 9.67E+03 0 0 -9.67E+03 0 0
(PERM)
Total use of renewable primary energy resources (PERT) MJ 1.44E+04 0 5.73E-01 2.07E+01 0 -1.2E+03
Non renewable primary energy as energy carrier (PENRE) MJ 4.06E+03 0 4.51E+01 1.92E+03 0 -1.46E+04
Non renewable primary energy as material utilization (PENRM) MJ 1.75E+03 0 0 -1.73E+03 0 0
Total use of non renewable primary energy resources (PENRT) MJ 5.81E+03 0 4.51E+01 1.95E+02 0 -1.46E+04
Use of secondary material (SM) kg 3.94E-03 0 0 0 0 0
Use of renewable secondary fuels (RSF) MJ 4.39E+02 0 0 0 0 7.85E+03
Use of non renewable secondary fuels (NRSF) MJ 0 0 0 0 0 1.4E+03
Use of net fresh water (FW) m3 6.7E+00 0 5.36E-03 1.08E-01 0 -5.9E+00
RESULTS OF THE LCA – WASTE CATEGORIES AND OUTPUT FLOWS according to EN 15804+A2:
1 m³ Unilin MDF Board
Parameter Unit A1-A3 C1 C2 C3 C4 D
Hazardous waste disposed (HWD) kg 9.9E+00 0 3.12E-02 2.9E-01 0 -2.25E+00
Non hazardous waste disposed (NHWD) kg 9.86E+01 0 4.44E+00 7.97E+00 0 -8.86E+01
Radioactive waste disposed (RWD) kg 3.87E-02 0 3.05E-04 1.36E-03 0 -5.8E-02
Components for re-use (CRU) kg 0 0 0 0 0 0
Materials for recycling (MFR) kg 0 0 0 0 0 0
Materials for energy recovery (MER) kg 0 0 0 6.37E+02 0 0
Exported electrical energy (EEE) MJ 0 0 0 0 0 0
Exported thermal energy (EET) MJ 0 0 0 0 0 0
RESULTS OF THE LCA – additional impact categories according to EN 15804+A2-optional:
1 m³ Unilin MDF Board
Parameter Unit A1-A3 C1 C2 C3 C4 D
7 Environmental Product Declaration - Unilin B.V. Division Panels - Unilin Medium Density Fiberboard
Disease
Incidence of disease due to PM emissions (PM) 9.55E-06 0 3.21E-07 7.13E-07 0 8.12E-06
incidence
Human exposure efficiency relative to U235 (IR) kBq U235 eq 3.01E+01 0 1.95E-01 1.33E+00 0 -6.68E+01
Comparative toxic unit for ecosystems (ETP-fw) CTUe 1.29E-04 0 5.52E-08 2.71E-07 0 -1.48E-06
Comparative toxic unit for humans (carcinogenic) (HTP-c) CTUh 9.9E-07 0 4.48E-10 3.02E-09 0 3.2E-08
Comparative toxic unit for humans (noncarcinogenic) (HTP-nc) CTUh 1.39E-07 0 1.25E-09 9.93E-09 0 -6.72E-08
Soil quality index (SQP) SQP 5.96E+04 0 5.15E+01 9.48E+01 0 -1.14E+03
Disclaimer 1 – for the indicator 'Potential Human exposure efficiency relative to U235'. This impact category deals mainly with the
eventual impact of low-dose ionizing radiation on human health of the nuclear fuel cycle. It does not consider effects due to possible
nuclear accidents, occupational exposure or radioactive waste disposal in underground facilities. Potential ionizing radiation from the
soil, radon and from some construction materials is also not measured by this indicator.
Disclaimer 2 – for the indicators 'abiotic depletion potential for non-fossil resources', 'abiotic depletion potential for fossil resources',
'water (user) deprivation potential, deprivation-weighted water consumption', 'potential comparative toxic unit for ecosystems', 'potential
comparative toxic unit for humans – cancerogenic', 'Potential comparative toxic unit for humans - not cancerogenic', 'potential soil
quality index'. The results of this environmental impact indicator shall be used with care as the uncertainties on these results are high
as there is limited experience with the indicator.
6. LCA: Interpretation
and stores it as biogenic carbon in its biomass. The product's
This section aims to analyze and interpret the results of the high wood content (i.e. 81 %) results in a GWP-total of - 765
LCA analysis carried for 1 m³ of the Unilin MDF board. The kg/m³. The product thus stores carbon and does not contribute
results refer to a product with a sales-weighted average to global warming when it leaves Unilin's factory gate. The
composition. Although the values for specific commercial stored carbon will only be released if the fiberboard can no
references can vary from the declared and discussed ones, the longer fulfill its intended purpose (i.e. at end of life).
observed trends will be the same throughout the entire product
category. A deep dive in the drivers of the cradle-to-gate environmental
impact shows the significant contribution of the raw materials
Summary (module A1). 74 % of the fossil CO emissions can primarily be
2
allocated to the (M)UF- and MDI-glue production, as well as 89
This part intends to summarize the trends observed in the % of the water used in A1 - A3. The generation of heat and
cradle-to-gate environmental impact of the Unilin raw electricity, required for the MDF production, is an important
fiberboard. An in-depth analysis is available in the following driver of the production-related impact. This is observable in the
subsections. EP and POCP indicators.
During its growth, wood absorbs CO through photosynthesis
2
biogenic = - 928 kg CO eq./m³). This negative GWP-value is
2
Cradle-to-Cradle Impact - Dominance Analysis partially counterbalanced by the positive GWP-impact of the
fossil materials and energy resources used during A1 - A3
The hot-spot analysis highlights the negative GWP-value of (GWP-fossil). This results in a GWP-total of - 765 kg CO
2
modules A1 - A3, as depicted in the GWP-focused graph. To
eq./m³ when the Unilin MDF board leaves the factory gate. The
improve the clarity of the graph, the values of the GWP-luluc
product under study thus stores carbon and does not contribute
indicator have been omitted.
to global warming.
Wood stores CO as biogenic carbon during its growth (GWP-
2 The stored carbon will only be released when the fiberboard
8 Environmental Product Declaration - Unilin B.V. Division Panels - Unilin Medium Density Fiberboard
leaves the system as a secondary fuel. The figure below clearly fossil CO emissions from combustion). It indicates that the
2
demonstrates a biogenic carbon balance in accordance with combustion of these fossil fuels has a higher impact on global
EN 16485. warming than the energy recovery from the secondary fuel.
The GWP-focused analysis also illustrates the "avoided" impact The hot-spot analysis shows that for non-GWP-related
(described in module D) related to the export of end-of-life parameters, modules A1 - A3 are the main contributors to the
fiberboard as a secondary fuel. The energy recovery of that fuel system under study. Values for module D are generally
generates heat and electricity, which substitutes a European- negative, except for the EP and POCP indicators. This is
averaged mix of heat and electricity from the grid. Since the attributed to the emissions from the energy recovery process of
largest share of the heat and electricity on the European grid is the end-of-life fiberboard.
fossil-based, a negative GWP-fossil is obtained (i.e. avoided
ODP, ADPE and WDP. 89 % of all water used in modules A1 -
Cradle-to-Grave Impact - Main Drivers A3 is allocated to the production of the raw materials (mainly
related to the glue production).
The graph below allows to identify the primary sources of the
cradle-to-gate environmental impact. The results show that raw Energy-related processes are typically the main drivers of the
material production (module A1) has a significant impact. 74 % environmental impact of module A3. This is observed in the
of the fossil CO emissions are primarily attributed to the contribution of A3 to EP and POCP, which is traced back to the
2
production of (M)-UF- and MDI-glue. The contribution of the raw generation of renewable heat from woody waste.
material production is even more significant for the indicators
9 Environmental Product Declaration - Unilin B.V. Division Panels - Unilin Medium Density Fiberboard
7. Requisite evidence
Formaldehyde emissions
• Test report : 220982-REQ1
E1 - EN 13986:2004+A1:2015
• Method : ASTM D6007-14
• Test report : QA-2022-1789 • Product : Fibralux FR
• Method : EN 717-1 • Laboratory : Wood.be
• Product : Fibrabel • Result : 0.06 ppm [Limit value < 0.11 ppm]
• Laboratory : WKI Fraunhofer
• Result : 0.04 ppm [Limit value < 0.1 ppm] PCP + Heavy metals + Wood preservative analysis
E0.5 - ChemVerbotsV As Unilin Fibreboard does not contain any post-consumer
recycling wood, this evidence is not necessary.
• Test report : 4022331076C_3-f-e
• Method : EN 717-1
• Product : Fibromax Pro LF+
VOC Emissions
• Laboratory : FCBA
• Result : 0.02 ppm [Limit value < 0.05 ppm]
Unspecified while raw fibreboards are always coated with a
finish in their end application. The type of finish (melamine,
CARB2/TSCA Title VI
paper foil, veneer, HPL,...) will determine the indoor air quality.
8. References
Standards EN 319
ASTM D6007 EN 319:1993, Particleboards and fibreboards - Determination
of tensile strength perpendicular to the plane of the board.
ASTM D6007:2020, Standard Test Method for Determining
Formaldehyde Concentrations in Air from Wood Products Using EN 322
a Small-Scale Chamber.
EN 322:1993, Wood-based panels - Determination of moisture
ASTM E1333 content.
ASTM E1333:2020, Standard Test Method for Determining EN 323
Formaldehyde Concentrations in Air and Emission Rates from
Wood Products Using a Large Chamber. EN 323:2005, Wood-based panels - Determination of density.
EN 310 EN 622
EN 310:1993, Wood-based panels - Determination of modulus EN 622-5:2010, Fibreboards - Specifications - Part 5:
of elasticity in bending and of bending strength. Requirements for dry process boards (MDF).
EN 317 EN 717-1
EN 317:1993, Particleboards and fibreboards; determination of EN 717-1:2004, Wood-based panels - Determination of
swelling in thickness after immersion in water; German version formaldehyde release Formaldehyde emission by the chamber
EN 317:1993. method
10 Environmental Product Declaration - Unilin B.V. Division Panels - Unilin Medium Density Fiberboard
EN 12460-5 ISO 45001
EN 12460-5:2015, Wood-based panels. Determination of EN ISO 45001:2018, Occupational health and safety
formaldehyde release Extraction method (called the perforator management systems — Requirements with guidance for use.
method).
ISO 50001
EN 13501-1
EN ISO 50001:2018, Energy management systems —
EN 13501-1:2007-05+A1:2009, Fire classification of Requirements with guidance for use.
construction products and building elements - Part 1:
classification with the results of tests on the reaction to fire of
building products. JIS A 1460
EN 13986 JIS A 1460:2021, Building boards Determination of
formaldehyde emission - Desiccator method.
EN 13986:2004+A1:2015, Wood-based panels for use in
construction— Characteristics, valuation of conformity and JIS A 5908
marking.
JIS A 5908:2022, Particleboards.
EN 15804
Additional References
EN 15804:2012+A2:2019+AC:2021, Sustainability of
construction works — Environmental Product Declarations — BBSR Table
Core rules for the product category of construction products.
BBSR 2017, Useful lives of building components for life cycle
EN 16449 analyses according to the Sustainable Building Assessment
System, 2017, BBSR Germany 2017.
EN 16449:2014, Wood and wood-based produts - Calculation
of the biogenic carbon content of wood and conversion to CPR
carbon dioxide.
CPR EU Ordinance No. 305/2011 of the European Parliament
EN 16485 and Council of 9th March 2011 to define harmonized conditions
for marketing building products.
EN 16485:2014, Round and sawn timber. Environmental
Product Declarations. Product category rules for wood and EcoInvent 3.8.
wood-based products for use in construction.
Ecoinvent 3.8, Database for Life Cycle Inventory and
EN 16516 Assessment. Swiss Centre for Life Cycle Inventories, 2021.
Available at: https://ecoinvent.org/the-ecoinvent-database/data-
EN 16516:2020, Construction products: Assessment of release releases/ecoinvent-3-8/.
of dangerous substances - Determination of emissions into
indoor air. EU Biocidal Products Ordinance No. 528/2012
ISO 9001 Regulation (EU) No 528/2012 of the European Parliament and
Council of 22 May 2012 concerning the making available on the
EN ISO 9001:2008-11, Quality Management Systems – market and use of biocidal products.
Requirements.
EWC
ISO 14001
European Waste Catalogue, Ordinance on the European Waste
EN ISO 14001:2015, Environmental management systems — Catalogue (Waste Catalogue Ordinance - AVV), reference
Requirements with guidance for use. Federal Official Journal I 2001, 3379.
ISO 14025 IBU 2022
EN ISO 14025:2011, Environmental labels and — Type III Institut Bauen und Umwelt e.V.: General Instructions for the
environmental declarations — Principles and procedures. EPD programme of Institut Bauen und Umwelt e.V., Version
2.1, Berlin: Institut Bauen und Umwelt e.V., 2022
ISO 14040 www.ibu-epd.com
EN ISO 14040:2006-10, Environmental management — Life PCR Part A
cycle assessment — Principles and framework.
Product Category Rules for Building-Related Products and
ISO 14044 Services. Part A: Calculation Rules for the Life Cycle
Assessment and Requirements on the Project Report according
ISO 14044:2006-10, Environmental management — Life cycle to EN 15804+A2:2019. Version 1.3. Berlin: Institut Bauen und
assessment — Principles and framework. Umwelt e.V. (eds.), 2021.
11 Environmental Product Declaration - Unilin B.V. Division Panels - Unilin Medium Density Fiberboard
PCR Part B SVHC List
Product Category Rules for Building-Related Products and List of Substances of Very High Concern (SVHC) Candidate for
Services. Part B: Requirements on the EPD for Wood based Authorisation (ECHA Candidate List), dated 04.07.2023,
panels. Version 2. Berlin: Institut Bauen und Umwelt e.V. (eds.), published in accordance with Article 59(10) of the REACH
2023. Regulation. Helsinki: European Chemicals Agency.
12 Environmental Product Declaration - Unilin B.V. Division Panels - Unilin Medium Density Fiberboard
Publisher
Institut Bauen und Umwelt e.V. +49 (0)30 3087748- 0
Hegelplatz 1 info@ibu-epd.com
10117 Berlin www.ibu-epd.com
Germany
Programme holder
Institut Bauen und Umwelt e.V. +49 (0)30 3087748- 0
Hegelplatz 1 info@ibu-epd.com
10117 Berlin www.ibu-epd.com
Germany
Author of the Life Cycle Assessment
Unilin B.V. Division Panels +32 56 67 52 11
Ooigemstraat 3 info.panels@unilin.com
8710 Wielsbeke https://www.unilinpanels.com/en-
Belgium gb
Owner of the Declaration
Unilin B.V. Division Panels +32 56 66 70 21
Ooigemstraat 3 info.panels@unilin.com
8710 Wielsbeke https://www.unilinpanels.com/en-
Belgium gb
13 Environmental Product Declaration - Unilin B.V. Division Panels - Unilin Medium Density Fiberboard
