ENVIRONMENTAL PRODUCT DECLARATION
as per ISO 14025 and EN 15804+A2
Owner of the Declaration dormakaba International Holding GmbH
Publisher Institut Bauen und Umwelt e.V. (IBU)
Programme holder Institut Bauen und Umwelt e.V. (IBU)
Declaration number EPD-DOR-20240049-CBA2-EN
Issue date 01.03.2024
Valid to 17.10.2027
Geryon Security Revolving Door
Dormakaba
www.ibu-epd.com | https://epd-online.com
General Information
Dormakaba Geryon Security Revolving Door
Programme holder Owner of the declaration
IBU – Institut Bauen und Umwelt e.V. dormakaba International Holding GmbH
Hegelplatz 1 DORMA Platz 1
10117 Berlin 58256 Ennepetal
Germany Germany
Declaration number Declared product / declared unit
EPD-DOR-20240049-CBA2-EN The declared unit is: one (1) dormakaba Geryon Security Revolving Door
(SRD-E01), consisting of the following items:
- drive and control unit (K8)
- upper body
- side walls
- columns incl. door leafs
- floor bearing
- fastening material
- packaging material
This declaration is based on the product category rules: Scope:
Electronic and physical Access Control Systems, 01.08.2021 This Environmental Product Declaration refers to a specific Geryon
(PCR checked and approved by the SVR) Security Revolving Door (SRD-E01) covering the variants 120° and 180°.
The products are manufactured at the dormakaba production facility in
Bühl (Germany).
Issue date Green electricity is being used at this production site.
01.03.2024
Data represents the year 2022.
The owner of the declaration shall be liable for the underlying information
and evidence; the IBU shall not be liable with respect to manufacturer
Valid to
information, life cycle assessment data and evidences.
17.10.2027
The EPD was created according to the specifications of EN 15804+A2. In
the following, the standard will be simplified as EN 15804.
Verification
The standard EN 15804 serves as the core PCR
Independent verification of the declaration and data according to ISO
14025:2011
internally X externally
Dipl.-Ing. Hans Peters
(Chairman of Institut Bauen und Umwelt e.V.)
Florian Pronold Dr.-Ing. Wolfram Trinius,
(Managing Director Institut Bauen und Umwelt e.V.) (Independent verifier)
1 Environmental Product Declaration - Dormakaba - Geryon Security Revolving Door
Product
• Option with in-built scales with weight limits or actual weight
Product description/Product definition • Option with night closure
Secure areas require a reliable system for identifying and • Option with optical separation using SRD Vision
separating authorized persons.
As these areas are usually representative of the building, a
secure but at the same time transparent access solution is Following technical data apply for Geryon Security
preferred. Revolving Door (SRD-E01):
Technical data
Geryon Security Revolving Door
Owing to the high transparency grade of the glass elements Name Value Unit
and a wide variety of colours for the metal parts, all models Outside diameter 1500-2000 mm
elegantly blend in with their surroundings. A sophisticated Total height 2300 mm
sensor system in compliance with the latest standards prevents
Passage height 2100 mm
users from being injured.
Upper part of body 200
Depending on the security requirements, the door may be
equipped with a contact mat, scales or internal monitoring. Number of door wings 3 or 4
Other variants are reinforced bullet- and burglar-resistant Rotary cycle 120° or 180°
designs, which are certified according to standards RC2 and Power supply 220-240 VAC
RC3 respectively. Options like a rotating unit with an Standby power consumption 60 VA
emergency exit function or a night closure complete the product
range. For the placing on the market in the European Product not harmonised in accordance with the CPR but in
Union/European Free Trade Associaton (EU/EFTA) (with the accordance with other provisions for harmonisation of the EU:
exception of Switzerland) the following legal provisions apply: • Machinery Directive 2006/42/EC
• Machinery Directive 2006/42/EC • 2014/30/EU Electromagnetic Compatibility Directive
• 2014/30/EU Electromagnetic Compatibility Directive • 2011/65/EU ROHS2 Directive
• 2011/65/EU ROHS2 Directive • DIN EN ISO 12100:2011-03 Safety of machinery
• DIN EN ISO 12100:2011-03 Safety of machinery • DIN EN 16005: 2013-01 and Amendment 2015-10
• DIN EN 16005: 2013-01 and Amendment 2015-10 Power operated pedestrian doorsets
Power operated pedestrian doorsets • DIN EN ISO 13849- 1:2016-06 Safety of machinery
• DIN EN ISO 13849- 1:2016-06 Safety of machinery • DIN EN ISO 13849- 2:2013-02 Safety of machinery
• DIN EN ISO 13849- 2:2013-02 Safety of machinery • DIN EN 60335-2-103: 2016-05 Household and similar
• DIN EN 60335-2-103: 2016-05 Household and similar electrical appliances
electrical appliances • DIN EN 61000-3-2:2015-03 Electromagnetic
• DIN EN 61000-3-2:2015-03 Electromagnetic compatibility (EMC)
compatibility (EMC) • DIN EN 61000-6-2: 2005 and Amendment:
• DIN EN 61000-6-2: 2005 and Amendment:2011 2011 Electromagnetic Compatibility (EMC)
Electromagnetic Compatibility (EMC) • DIN EN 61000-6-3:2007 and A1:2011 Electromagnetic
• DIN EN 61000-6-3:2007 and A1:2011 Electromagnetic Compatibility (EMC)
Compatibility (EMC)
Base materials/Ancillary materials
The CE-marking takes into account the proof of conformity with
The major material composition including packaging is listed
the respective harmonized standards based on the legal
below:
provisions above.
For the application and use the respective national provisions Name Value Unit
apply. Glass 40 %
Aluminium 32 %
Application
Steel 20 %
For secure entry to:
Plastic 6 %
• Sensitive areas in administrative buildings,
Electronics 1,5 %
industrial premises, government agencies and
ministries Paper 1 %
• Banks and financial institutions Copper 0,5 %
• Data and research centres
The product contains partial articles which contain substances
• Staff entrances at airports
listed in the Candidate List of REACH Regulation
• Nuclear power plants
1907/2006/EC (date: 10.06.2022) exceeding 0.1 percentage by
Technical Data mass: no
Key elements and options of the Geryon Security
The Candidate List can be found on the ECHA website
Revolving Door:
address: https://echa.europa.eu/de/home.
• Users cannot become stuck thanks to end point locking Reference service life
• Safety sensor system according to DIN EN 16005
The reference service life amounts to 20 years and depends on
• Standard version has IR sensor system
the application and frequency of use. For repairs and renewals,
• Versions with resistance classes RC2 and RC3
suitable spare pars are available. The Geryon Security
• All-glass units with underfloor drive
Revolving Door is tested to EN 16005.
• Option with approved emergency exit column
2 Environmental Product Declaration - Dormakaba - Geryon Security Revolving Door
LCA: Calculation rules
Declared Unit End-of-life stage– Modules C1-C4 and D
The declared unit is 1 piece of product: 459 kg The end-of-life stage includes:
Declared unit — C1, de-construction, demolition:
— C2, transport to waste processing;
Name Value Unit
— C3, waste processing for reuse, recovery and/or recycling;
Declared unit 1 pce.
— C4, disposal;
Mass (total system excluding packaging)) 459 kg including provision and all transport, provision of all materials,
products and related energy and water use.
System boundary
Type of EPD: cradle to gate with options, modules C1–C4, and Module D (Benefits and loads beyond the system boundary)
module D (A1–A3 + C + D and additional modules: A4 + A5 + includes:
B6) — D, recycling potentials, expressed as net impacts and
benefits.
Production - Module A1-A3
Geographic Representativeness
The product stage includes:
Land or region, in which the declared product system is
— A1, raw material extraction, processing and mechanical
manufactured, used or handled at the end of the product´s
treatments, processing of secondary material input (e.g.
lifespan: Germany
recycling processes), — A2, transport to the manufacturer,
— A3, manufacturing and assembly including provision of all
materials, products and energy, as well as waste processing up
Comparability
to the end-of-waste state.
Basically, a comparison or an evaluation of EPD data is only
possible if all the data sets to be compared were created
Construction stage - Modules A4-A5
according to EN 15804 and the building context, respectively
The construction process stage includes:
the product-specific characteristics of performance, are taken
— A4, transport to the building site;
into account.
— A5, installation into the building;
including provision of all materials, products and energy, as well
as waste processing up to the end-of-waste state or disposal of
final residues during the construction process stage.
Use stage - Module B6
The use stage related to the operation of the building includes:
— B6, operational energy use.
The potential use of electricity from the grid is declared in
module B6.
LCA: Scenarios and additional technical information
Name Value Unit
Characteristic product properties of biogenic carbon
Waste packaging (paper and plastic) kg
Information on describing the biogenic Carbon Content at
factory gate Reference service life
Name ValueUnit Name Value Unit
kg Life Span according to the manufacturer 20 a
Biogenic carbon content in product 0.26
C
Operational energy use (B6)
Biogenic carbon content in accompanying kg
1.47 The use stage is declared for 20 years
packaging C
Name Value Unit
Days per year in use 365 days
The following technical scenario information is required for the
declared modules On mode per day 1 hours
Idle mode per day 15 hours
Transport to the building site (A4)
Off mode 8 hours
Name Value Unit
On mode power 36 W
Litres of fuel (per 1 kg) 0.00276l/100km
Idle mode power 22 W
Transport distance via medium truck 100 km
Off mode power 0 W
Capacity utilisation (including empty runs) via
55 %
medium truck Electricity consumption per 1 year 131 kWh
Transport distance is declared for a distance of 100km by truck End of life (C1-C4)
in order to allow scaling to a specific point of installation.
C1: The product dismantling from the building is done manually
without environmental burden.
Installation into the building (A5) C2: Transport to waste treatment at end of life is 50 km.
3 Environmental Product Declaration - Dormakaba - Geryon Security Revolving Door
Name Value Unit Reuse, recovery and/or recycling potentials (D), relevant
Collected separately waste type waste type 459 kg scenario information
Reuse - kg Collection rate is 100%.
Recycling 243 kg Name Value Unit
Energy recovery 26 kg Recycling 100 %
Landfilling 190 kg
The product is disassembled in a recycling process. Material
recycling is then assumed for the metals, and electronics. The
plastic components are assumed to be incinerated with energy
recovery. Glass, electromechanics and batteries are assumed
to be landfilled. Region for the End of Life is: Global.
4 Environmental Product Declaration - Dormakaba - Geryon Security Revolving Door
LCA: Results
DESCRIPTION OF THE SYSTEM BOUNDARY (X = INCLUDED IN LCA; MND = MODULE OR INDICATOR NOT DECLARED; MNR
= MODULE NOT RELEVANT)
Benefits and
Construction loads beyond
Product stage Use stage End of life stage
process stage the system
boundaries
la ire ta m w a Ry lp p u s tro p s n a rT g n iru tc a fu n a M e h t m o rf tro p s n a rTe tis e h t o t e ta g y lb m e s s A e s U e c n a n e tn ia M ria p e R tn e m e c a lp e R tn e m h s ib ru fe R y g re n e la n o ita re p Oe s u re ta w la n o ita re p Oe s u n o itc u rts n o c -e Dn o itilo m e d tro p s n a rT g n is s e c o rp e ts a W la s o p s iD -e s u e R-y re v o c e R-g n ilc y c e Rla itn e to p
A1 A2 A3 A4 A5 B1 B2 B3 B4 B5 B6 B7 C1 C2 C3 C4 D
X X X X X MND X MNR MNR MNR X MND X X X X X
RESULTS OF THE LCA - ENVIRONMENTAL IMPACT according to EN 15804+A2: 1 piece Geryon SRD
Parameter Unit A1-A3 A4 A5 B2 B6 C1 C2 C3 C4 D
GWP-total kg CO 2 eq 2.04E+03 4.06E+00 5.67E+00 0 1.06E+03 0 2.01E+00 6.77E+01 2.9E+00 -1.05E+03
GWP-fossil kg CO 2 eq 2.05E+03 3.88E+00 1.42E-01 0 1.05E+03 0 1.92E+00 6.65E+01 2.89E+00 -1.05E+03
GWP-
biogenic kg CO 2 eq -5.5E+00 1.79E-01 5.53E+00 0 3.52E+00 0 8.9E-02 1.19E+00 1E-02 -2.99E+00
GWP-luluc kg CO 2 eq 9.72E-01 9.23E-05 9.33E-05 0 1.53E+00 0 4.57E-05 4E-03 8E-03 -1.94E-01
ODP kg CFC11 eq 6.48E-09 4.1E-16 1.02E-15 0 2.32E-11 0 2.03E-16 3.37E-14 1.07E-14 -7.33E-09
AP mol H+ eq 1.02E+01 4E-03 2E-03 0 2.33E+00 0 2E-03 1.2E-02 2.1E-02 -3.89E+00
EP-
kg P eq 2.21E-03 8.3E-07 2E-07 0 3E-03 0 4.11E-07 5.37E-06 4.96E-06 -5.5E-04
freshwater
EP-marine kg N eq 1.64E+00 1E-03 5.74E-04 0 5.17E-01 0 6.12E-04 3E-03 5E-03 -5.15E-01
EP-terrestrial mol N eq 1.81E+01 1.4E-02 7E-03 0 5.43E+00 0 7E-03 5.5E-02 5.9E-02 -5.56E+00
kg NMVOC
POCP 4.56E+00 3E-03 2E-03 0 1.42E+00 0 2E-03 8E-03 1.6E-02 -1.66E+00
eq
ADPE kg Sb eq 2.7E-02 1.16E-07 1.61E-08 0 3.05E-04 0 5.76E-08 4.62E-07 2.59E-07 -9E-03
ADPF MJ 2.7E+04 5.5E+01 1.79E+00 0 1.85E+04 0 2.72E+01 3.11E+01 3.79E+01 -1.44E+04
m3 world eq
WDP 2.48E+02 8E-03 7.03E-01 0 2.3E+02 0 4E-03 6.93E+00 3.03E-01 -6.02E+01
deprived
GWP = Global warming potential; ODP = Depletion potential of the stratospheric ozone layer; AP = Acidification potential of land and water; EP =
Eutrophication potential; POCP = Formation potential of tropospheric ozone photochemical oxidants; ADPE = Abiotic depletion potential for non-fossil
resources; ADPF = Abiotic depletion potential for fossil resources; WDP = Water (user) deprivation potential)
RESULTS OF THE LCA - INDICATORS TO DESCRIBE RESOURCE USE according to EN 15804+A2: 1 piece Geryon SRD
Parameter Unit A1-A3 A4 A5 B2 B6 C1 C2 C3 C4 D
PERE MJ 8.68E+03 1.73E-01 4.83E+01 0 8.22E+03 0 8.6E-02 1.73E+01 4.96E+00 -6.29E+03
PERM MJ 5.72E+01 0 -4.8E+01 0 0 0 0 -9.24E+00 0 0
PERT MJ 8.74E+03 1.73E-01 3.25E-01 0 8.22E+03 0 8.6E-02 8.07E+00 4.96E+00 -6.29E+03
PENRE MJ 2.61E+04 5.51E+01 1.79E+00 0 1.85E+04 0 2.73E+01 8.72E+02 3.79E+01 -1.44E+04
PENRM MJ 8.41E+02 0 0 0 0 0 0 -8.41E+02 0 0
PENRT MJ 2.7E+04 5.51E+01 1.79E+00 0 1.85E+04 0 2.73E+01 3.11E+01 3.79E+01 -1.44E+04
SM kg 3.06E+01 0 0 0 0 0 0 0 0 0
RSF MJ 0 0 0 0 0 0 0 0 0 0
NRSF MJ 0 0 0 0 0 0 0 0 0 0
FW m3 2.07E+01 3.11E-04 1.7E-02 0 9.5E+00 0 1.54E-04 1.66E-01 1E-02 -1.14E+01
PERE = Use of renewable primary energy excluding renewable primary energy resources used as raw materials; PERM = Use of renewable primary
energy resources used as raw materials; PERT = Total use of renewable primary energy resources; PENRE = Use of non-renewable primary energy
excluding non-renewable primary energy resources used as raw materials; PENRM = Use of non-renewable primary energy resources used as raw
materials; PENRT = Total use of non-renewable primary energy resources; SM = Use of secondary material; RSF = Use of renewable secondary fuels;
NRSF = Use of non-renewable secondary fuels; FW = Use of net fresh water
RESULTS OF THE LCA – WASTE CATEGORIES AND OUTPUT FLOWS according to EN 15804+A2:
1 piece Geryon SRD
Parameter Unit A1-A3 A4 A5 B2 B6 C1 C2 C3 C4 D
HWD kg 6.37E-05 5.34E-09 2.64E-09 0 7.68E-06 0 2.64E-09 1.18E-07 5.77E-07 -1.3E-04
NHWD kg 4.24E+02 6E-03 1.78E-01 0 1.32E+01 0 3E-03 6.92E+00 1.9E+02 -2.37E+02
RWD kg 1.26E+00 5.91E-05 9.41E-05 0 2.81E+00 0 2.93E-05 1E-03 4.31E-04 -1.5E+00
CRU kg 0 0 0 0 0 0 0 0 0 0
MFR kg 0 0 0 0 0 0 0 2.42E+02 0 0
MER kg 0 0 0 0 0 0 0 0 0 0
EEE MJ 0 0 8.58E+00 0 0 0 0 0 0 0
5 Environmental Product Declaration - Dormakaba - Geryon Security Revolving Door
EET MJ 0 0 1.56E+01 0 0 0 0 0 0 0
HWD = Hazardous waste disposed; NHWD = Non-hazardous waste disposed; RWD = Radioactive waste disposed; CRU = Components for re-use;
MFR = Materials for recycling; MER = Materials for energy recovery; EEE = Exported electrical energy; EET = Exported thermal energy
RESULTS OF THE LCA – additional impact categories according to EN 15804+A2-optional:
1 piece Geryon SRD
Parameter Unit A1-A3 A4 A5 B2 B6 C1 C2 C3 C4 D
Disease
PM 9.7E-05 2.04E-08 8.8E-09 0 1.95E-05 0 1.01E-08 1.52E-07 2.56E-07 -6.17E-05
incidence
IR kBq U235 eq 2.42E+02 8E-03 1.5E-02 0 4.62E+02 0 4E-03 1.05E-01 4.4E-02 -3.01E+02
ETP-fw CTUe 1.42E+04 3.9E+01 8.5E-01 0 7.93E+03 0 1.93E+01 1.17E+01 2.16E+01 -5.14E+03
HTP-c CTUh 8.51E-06 7.33E-10 4.49E-11 0 2.19E-07 0 3.63E-10 1.01E-09 3.21E-09 -2.48E-07
HTP-nc CTUh 2.59E-05 3.14E-08 1.95E-09 0 8.07E-06 0 1.55E-08 1.02E-07 3.53E-07 -8.19E-06
SQP SQP 3.06E+03 1.41E-01 4.75E-01 0 5.91E+03 0 7E-02 9.31E+00 7.9E+00 -4.93E+02
PM = Potential incidence of disease due to PM emissions; IR = Potential Human exposure efficiency relative to U235; ETP-fw = Potential comparative
Toxic Unit for ecosystems; HTP-c = Potential comparative Toxic Unit for humans (cancerogenic); HTP-nc = Potential comparative Toxic Unit for humans
(not cancerogenic); SQP = Potential soil quality index
Disclaimer 1 – for the indicator 'Potential Human exposure efficiency relative to U235'. This impact category deals mainly with the
eventual impact of low-dose ionizing
radiation on human health of the nuclear fuel cycle. It does not consider effects due to possible nuclear accidents, occupational
exposure or radioactive waste disposal in underground facilities. Potential ionizing radiation from the soil, radon and from some
construction materials is also not measured by this indicator.
Disclaimer 2 – for the indicators 'abiotic depletion potential for non-fossil resources', 'abiotic depletion potential for fossil resources',
'water (user) deprivation potential, deprivation-weighted water consumption', 'potential comparative toxic unit for ecosystems', 'potential
comparative toxic unit for humans –
cancerogenic', 'Potential comparative toxic unit for humans - not cancerogenic', 'potential soil quality index'. The results of this
environmental impact indicator shall be used with care as the uncertainties on these results are high as there is limited experience with
the indicator. This EPD was created using a software tool.
References
DIN EN 16005 ISO 14025
DIN EN 16005: 2013-01 and Amendment 2015-10 DIN EN ISO 14025:2011-10, Environmental labels and
Power operated pedestrian doorsets declarations — Type III environmental declarations —
Principles and procedures.
DIN EN 60335-2
DIN EN 60335-2-103: 2016-05 Household and similar 2014/30/EU Electromagnetic Compatibility Directive
electrical appliances DIRECTIVE 2014/30/EU OF THE EUROPEAN
PARLIAMENT AND OF THE COUNCIL of 26 February
DIN EN 61000-3-2 2014 on the harmonisation of the laws of the Member
DIN EN 61000-3-2: 201503 Electromagnetic compatibility States relating to electromagnetic compatibility
(EMC)
European Waste Catalogue (EWC)
DIN EN 61000-6-2 COMMISSION DECISION of 18 December 2014
DIN EN 61000-6-2: 2005 and Amendment:2011 amending Decision 2000/532/EC on the list of waste
Electromagnetic Compatibility (EMC) pursuant to Directive 2008/98/EC of the European
Parliament and of the Council
DIN EN 61000-6-3
DIN EN 61000-6-3: 2007 and A1:2011 Electromagnetic Machinery Directive 2006/42/EC
Compatibility (EMC) DIRECTIVE 2006/42/EC OF THE EUROPEAN
PARLIAMENT AND OF THE COUNCIL of 17 May
DIN EN ISO 12100 2006 on machinery, and amending Directive 95/16/EC
DIN EN ISO 12100:2011-03 Safety of machinery
REACH
DIN EN ISO 13849- 1 Regulation (EC) No 1907/2006 of the European
DIN EN ISO 13849-1: 2016-06 Safety of machinery Parliament and of the Council on the Registration,
Evaluation, Authorisation and Restriction of Chemicals
DIN EN ISO 13849- 2 (REACH)
DIN EN ISO 13849-2: 2013-02 Safety of machinery
ROHS2 Directive
EN 15804 Directive 2011/65/EU of the European Parliament and
EN 15804+A2, Sustainability of of the Council of 8 June 2011 on the restriction of the
construction works - Environmental Product use of certain hazardous substances in electrical and
Declarations - Core rules for the product category of electronic equipment
construction products.
ISO 9001
ISO 9001:2015-09 Quality management systems Requirements
6 Environmental Product Declaration - Dormakaba - Geryon Security Revolving Door
Further References LCA-tool dormakaba
LCA tool, ESC (Entrance System Control)
IBU 2021 Tool No.: IBU-DOR-202109-LT1-EN
General Instructions for the EPD programme of Institut Bauen Developed by Sphera Solutions GmbH.
und Umwelt e.V. Version 2.0, Berlin: Institut Bauen und Umwelt
e.V., 2021 www.ibu-epd.com PCR Part A
PCR – Part A: Calculation Rules for the Life Cycle
GaBi ts software Assessment and Requirements on the Project Report
Sphera Solutions GmbH Gabi Software System and according to EN 15804+A2:2019, Version 1.0, Institut
Database for Life Cycle Engineering 19922020 Bauen und Umwelt e.V., www.ibu-epd.com.
Version 10.0.0.71 University of Stuttgart
Leinfelden-Echterdingen PCR Part B
PCR – Part B: Requirements on the EPD for electronic
GaBi ts documentation and physical Access Control Systems, version 08/2021,
GaBi life cycle inventory data documentation Institut Bauen und Umwelt e.V., www.ibu-epd.com.
(https://www.gabisoftware.
com/support/gabi/gabidatabase[1]2020lcidocumentati
on/).
7 Environmental Product Declaration - Dormakaba - Geryon Security Revolving Door
Publisher
Institut Bauen und Umwelt e.V. +49 (0)30 3087748- 0
Hegelplatz 1 info@ibu-epd.com
10117 Berlin www.ibu-epd.com
Germany
Programme holder
Institut Bauen und Umwelt e.V. +49 (0)30 3087748- 0
Hegelplatz 1 info@ibu-epd.com
10117 Berlin www.ibu-epd.com
Germany
Author of the Life Cycle Assessment
dormakaba International Holding GmbH +49 2333 793-0
DORMA Platz 1 info.de@dormakaba.com
58256 Ennepetal www.dormakaba.com
Germany
Owner of the Declaration
dormakaba International Holding GmbH +49 2333 793-0
DORMA Platz 1 info.de@dormakaba.com
58256 Ennepetal www.dormakaba.com
Germany
8 Environmental Product Declaration - Dormakaba - Geryon Security Revolving Door
