ENVIRONMENTAL PRODUCT DECLARATION
as per ISO 14025 and EN 15804+A2
Owner of the Declaration dormakaba International Holding GmbH
Publisher Institut Bauen und Umwelt e.V. (IBU)
Programme holder Institut Bauen und Umwelt e.V. (IBU)
Declaration number EPD-DOR-20220068-CBA7-EN
Issue date 04.05.2022
Valid to 03.05.2027
TS 90 Impulse
dormakaba
www.ibu-epd.com | https://epd-online.com
General Information
dormakaba TS 90 Impulse
Programme holder Owner of the declaration
IBU – Institut Bauen und Umwelt e.V. dormakaba International Holding GmbH
Hegelplatz 1 DORMA Platz 1
10117 Berlin 58256 Ennepetal
Germany Germany
Declaration number Declared product / declared unit
EPD-DOR-20220068-CBA7-EN 1 door closer (1 piece) TS 90 Impulse
This declaration is based on the product category rules: Scope:
Building Hardware products, 01.08.2021 This Environmental Product Declaration refers to a specific door closer
(PCR checked and approved by the SVR) manufactured by dormakaba Production GmbH & Co. KG. The production
site is located in Singapore.
Issue date The data represents the year 2020.
The owner of the declaration shall be liable for the underlying information
04.05.2022
and evidence; the IBU shall not be liable with respect to manufacturer
information, life cycle assessment data and evidences.
Valid to
The EPD was created according to the specifications of EN 15804+A2. In
03.05.2027 the following, the standard will be simplified as EN 15804.
Verification
The standard EN 15804 serves as the core PCR
Independent verification of the declaration and data according to ISO
14025:2011
internally X externally
Dipl.-Ing. Hans Peters
(Chairman of Institut Bauen und Umwelt e.V.)
Florian Pronold Dr.-Ing. Wolfram Trinius,
(Managing Director Institut Bauen und Umwelt e.V.) (Independent verifier)
1 Environmental Product Declaration - dormakaba - TS 90 Impulse
Product
Performance data of the product with respect to its
Product description/Product definition characteristics in accordance with the relevant technical
TS 90 Impulse combines technical superiority with outstanding provision which can be applied are mentioned above.
value, and unites advanced design with convenient
functionality - all on the basis of its heart-shaped cam. Two Base materials/Ancillary materials
regulating valves for precise adjustment of closing speed and The major material compositions including the packaging of the
available accessories makes the TS 90 a versatile and cost- product are listed below:
efficient choice for interior doors. The TS 90 is non-handed and Name Value Unit
offers easy and universal installation in all four mounting
Steel 46 %
positions without mounting plate. Ease-of-use is also
Paper 24 %
underlined by the ready-to-install complete packaging that
simplifies stock keeping and processing on site. For the use Aluminium 23 %
and application of the product the respective national provisions Lubricant 3 %
at the place of use apply. The standards which can be applied Plastics 1 %
are the following:
Zinc 1 %
Others 2 %
• EN 1154
The product includes partial articles which contain substances
• EN 1634-1
listed in the Candidate List of REACH Regulation
Application 1907/2006/EC (date: 17.01.2022) exceeding 0.1 percentage by
With its installation versatility and inherent functional reliability, mass: yes
it is ideal for virtually any application.
• Lead (Pb): 7439-92-1 (CAS-No.) is included in some of
Technical Data
the alloys used. The concentration of lead in each
The door closer has following technical properties:
individual alloy does not exceed 4.0% (by mass).
The Candidate List can be found on the ECHA website
address: https:echa.europa.eu/de/home.
Reference service life
The reference service life of the TS 90 Impulse door closer
depends on the traffic pattern and degree of usage of the door.
These closers are rated to EN 1154, meaning they are
designed to withstand a minimum of 500,000 cycles. The
reference service life amounts for 20 years. This corresponds
with approx. 25,000 cycles per year.
LCA: Calculation rules
Declared Unit Production - Module A1-A3
The declared unit is 1 piece of the product: TS 90 Impulse. The product stage includes:
Name Value Unit — A1, raw material extraction, processing and mechanical
Declared unit 1 piece/product treatments, processing of secondary material input (e.g.
recycling processes),
Mass of declared Product 2.5 kg
— A2, transport to the manufacturer,
— A3, manufacturing and assembly including provision of all
System boundary
materials, products and energy, as well as waste processing up
The type of EPD is: cradle to gate with options, modules C1–
to the end-of waste state.
C4, and module D (A1–A3 + C + D and additional modules: A4
+ A5)
Construction stage - Modules A4-A5
2 Environmental Product Declaration - dormakaba - TS 90 Impulse
The construction process stage includes: — D, recycling potentials, expressed as net impacts and
— A4, transport to the building site; benefits.
— A5, installation into the building; including provision of all
materials, products and energy, as well as waste processing up Geographic Representativeness
to the end-of waste state or disposal of final residues during the Land or region, in which the declared product system is
construction process stage. manufactured, used or handled at the end of the product´s
lifespan: Singapore
End-of-life stage– Modules C1-C4 and D
The end-of-life stage includes:
Comparability
— C1, de-construction, demolition:
Basically, a comparison or an evaluation of EPD data is only
— C2, transport to waste processing;
possible if all the data sets to be compared were created
— C3, waste processing for reuse, recovery and/or recycling;
according to EN 15804 and the building context, respectively
— C4, disposal; including provision and all transport, provision
the product-specific characteristics of performance, are taken
of all materials, products and related energy and water use.
into account.
Module D (Benefits and loads beyond the system boundary)
includes:
LCA: Scenarios and additional technical information
Reference service life
Characteristic product properties of biogenic carbon
Name Value Unit
Information on describing the biogenic Carbon Content at
Life Span according to the manufacturer 20 a
factory gate
Name ValueUnit End of life (C1-C4)
Biogenic carbon content in accompanying kg C1: The product dismantling from the building is done manually
0.21
packaging C without environmental burden.
C2: Transport to waste treatment at end of life is 50km.
Additional technical information for the declared modules. Name Value Unit
Transport to the building site (A4) Collected separately waste type 1.92 kg
Recycling 1.77 kg
Name Value Unit
Energy recovery 0.019 kg
Litres of fuel truck (per piece) 0.00276l/100km
Final deposition 0,13 kg
Transport distance (truck) 750 km
Capacity utilisation (including empty runs) 55 % Reuse, recovery and/or recycling potentials (D), relevant
average scenario information
Transport distance (ship) 17300 km
Name Value Unit
Installation into the building (A5) Recycling 100 %
Name ValueUnit Collection rate is 100%.
Output substances following waste treatment on
0.58 kg
site (paper packaging)
3 Environmental Product Declaration - dormakaba - TS 90 Impulse
LCA: Results
DESCRIPTION OF THE SYSTEM BOUNDARY (X = INCLUDED IN LCA; MND = MODULE OR INDICATOR NOT DECLARED; MNR
= MODULE NOT RELEVANT)
Benefits and
Construction loads beyond
Product stage Use stage End of life stage
process stage the system
boundaries
la ire ta m w a Ry lp p u s tro p s n a rT g n iru tc a fu n a M e h t m o rf tro p s n a rTe tis e h t o t e ta g y lb m e s s A e s U e c n a n e tn ia M ria p e R tn e m e c a lp e R tn e m h s ib ru fe R y g re n e la n o ita re p Oe s u re ta w la n o ita re p Oe s u n o itc u rts n o c -e Dn o itilo m e d tro p s n a rT g n is s e c o rp e ts a W la s o p s iD -e s u e R-y re v o c e R-g n ilc y c e Rla itn e to p
A1 A2 A3 A4 A5 B1 B2 B3 B4 B5 B6 B7 C1 C2 C3 C4 D
X X X X X MND MND MNR MNR MNR MND MND X X X X X
RESULTS OF THE LCA - ENVIRONMENTAL IMPACT according to EN 15804+A2: 1 door closer
Parameter Unit A1-A3 A4 A5 C1 C2 C3 C4 D
GWP-total kg CO 2 eq 7.5E+00 3.05E-01 8.25E-01 0 8E-03 4.8E-02 2E-03 -3.93E+00
GWP-fossil kg CO 2 eq 8.42E+00 2.98E-01 2.1E-02 0 8E-03 4.8E-02 2E-03 -3.92E+00
GWP-biogenic kg CO 2 eq -9.3E-01 7E-03 8.04E-01 0 3.63E-04 1.13E-06 6.84E-06 -1.2E-02
GWP-luluc kg CO 2 eq 6E-03 6.64E-06 1.36E-05 0 1.87E-07 2.73E-06 5.76E-06 -7.54E-04
ODP kg CFC11 eq 3.82E-11 2.99E-17 1.49E-16 0 8.3E-19 2.44E-17 7.42E-18 -2.93E-11
AP mol H+ eq 3.6E-02 5E-03 2.31E-04 0 7.87E-06 8.6E-06 1.44E-05 -1.4E-02
EP-freshwater kg P eq 2.27E-05 6.54E-08 2.91E-08 0 1.68E-09 3.89E-09 3.44E-09 -2.28E-06
EP-marine kg N eq 6.29E-03 1E-03 8.34E-05 0 2.5E-06 1.94E-06 3.7E-06 -2E-03
EP-terrestrial mol N eq 6.6E-02 1.6E-02 1E-03 0 2.78E-05 3.92E-05 4.06E-05 -2.1E-02
kg NMVOC
POCP 1.88E-02 4E-03 2.21E-04 0 7.08E-06 5.37E-06 1.12E-05 -6E-03
eq
ADPE kg Sb eq 1.38E-04 8.33E-09 2.35E-09 0 2.36E-10 3.34E-10 1.8E-10 -2.24E-05
ADPF MJ 1.16E+02 3.93E+00 2.61E-01 0 1.11E-01 2.2E-02 2.6E-02 -5.68E+01
m3 world eq
WDP 1.2E+00 5.61E-04 1.02E-01 0 1.54E-05 5E-03 2.1E-04 -1.95E-01
deprived
GWP = Global warming potential; ODP = Depletion potential of the stratospheric ozone layer; AP = Acidification potential of land and water; EP =
Eutrophication potential; POCP = Formation potential of tropospheric ozone photochemical oxidants; ADPE = Abiotic depletion potential for non-fossil
resources; ADPF = Abiotic depletion potential for fossil resources; WDP = Water (user) deprivation potential)
RESULTS OF THE LCA - INDICATORS TO DESCRIBE RESOURCE USE according to EN 15804+A2: 1 door closer
Parameter Unit A1-A3 A4 A5 C1 C2 C3 C4 D
PERE MJ 4.65E+01 1.3E-02 7.03E+00 0 3.52E-04 1.5E-01 3E-03 -2.6E+01
PERM MJ 7.13E+00 0 -6.98E+00 0 0 -1.44E-01 0 0
PERT MJ 5.37E+01 1.3E-02 4.7E-02 0 3.52E-04 6E-03 3E-03 -2.6E+01
PENRE MJ 1.15E+02 3.94E+00 2.61E-01 0 1.12E-01 7.09E-01 2.6E-02 -5.68E+01
PENRM MJ 6.87E-01 0 0 0 0 -6.87E-01 0 0
PENRT MJ 1.16E+02 3.94E+00 2.61E-01 0 1.12E-01 2.2E-02 2.6E-02 -5.68E+01
SM kg 1.19E+00 0 0 0 0 0 0 0
RSF MJ 0 0 0 0 0 0 0 0
NRSF MJ 0 0 0 0 0 0 0 0
FW m3 9.1E-02 2.28E-05 2E-03 0 6.31E-07 1.18E-04 6.63E-06 -4.5E-02
PERE = Use of renewable primary energy excluding renewable primary energy resources used as raw materials; PERM = Use of renewable primary
energy resources used as raw materials; PERT = Total use of renewable primary energy resources; PENRE = Use of non-renewable primary energy
excluding non-renewable primary energy resources used as raw materials; PENRM = Use of non-renewable primary energy resources used as raw
materials; PENRT = Total use of non-renewable primary energy resources; SM = Use of secondary material; RSF = Use of renewable secondary fuels;
NRSF = Use of non-renewable secondary fuels; FW = Use of net fresh water
RESULTS OF THE LCA – WASTE CATEGORIES AND OUTPUT FLOWS according to EN 15804+A2:
1 door closer
Parameter Unit A1-A3 A4 A5 C1 C2 C3 C4 D
HWD kg 1.44E-06 3.84E-10 3.84E-10 0 1.08E-11 8.53E-11 4.01E-10 -1.11E-07
NHWD kg 1.54E+00 4.03E-04 2.6E-02 0 1.14E-05 5E-03 1.32E-01 -9.71E-01
RWD kg 5E-03 4.3E-06 1.37E-05 0 1.2E-07 8.31E-07 2.99E-07 -6E-03
CRU kg 0 0 0 0 0 0 0 0
MFR kg 0 0 0 0 0 1.73E+00 0 0
MER kg 0 0 0 0 0 0 0 0
EEE MJ 0 0 1.25E+00 0 0 0 0 0
EET MJ 0 0 2.26E+00 0 0 0 0 0
HWD = Hazardous waste disposed; NHWD = Non-hazardous waste disposed; RWD = Radioactive waste disposed; CRU = Components for re-use;
MFR = Materials for recycling; MER = Materials for energy recovery; EEE = Exported electrical energy; EET = Exported thermal energy
4 Environmental Product Declaration - dormakaba - TS 90 Impulse
RESULTS OF THE LCA – additional impact categories according to EN 15804+A2-optional:
1 door closer
Parameter Unit A1-A3 A4 A5 C1 C2 C3 C4 D
Disease
PM 3.98E-07 8.98E-08 1.28E-09 0 4.14E-11 1.1E-10 1.78E-10 -2.28E-07
incidence
IR kBq U235 eq 1.06E+00 6.16E-04 2E-03 0 1.71E-05 7.49E-05 3.08E-05 -1.25E+00
ETP-fw CTUe 3.91E+01 2.79E+00 1.24E-01 0 7.9E-02 8E-03 1.5E-02 -2.08E+01
HTP-c CTUh 4.26E-09 5.24E-11 6.54E-12 0 1.49E-12 7.27E-13 2.22E-12 -7.81E-10
HTP-nc CTUh 1.12E-07 2.35E-09 2.83E-10 0 6.36E-11 7.37E-11 2.45E-10 -5.1E-09
SQP SQP 1.21E+02 1E-02 6.9E-02 0 2.87E-04 7E-03 5E-03 -2.2E+00
PM = Potential incidence of disease due to PM emissions; IR = Potential Human exposure efficiency relative to U235; ETP-fw = Potential comparative
Toxic Unit for ecosystems; HTP-c = Potential comparative Toxic Unit for humans (cancerogenic); HTP-nc = Potential comparative Toxic Unit for humans
(not cancerogenic); SQP = Potential soil quality index
Disclaimer 1 – for the indicator “Potential Human exposure efficiency relative to U235”. This impact category deals mainly with the
eventual impact of low-dose ionizing radiation on human health of the nuclear fuel cycle. It does not consider effects due to possible
nuclear accidents, occupational exposure or radioactive waste disposal in underground facilities. Potential ionizing radiation from the
soil, radon and from some construction materials is also not measured by this indicator.
Disclaimer 2 – for the indicators “abiotic depletion potential for non-fossil resources”, “abiotic depletion potential for fossil resources”,
“water (user) deprivation potential, deprivation-weighted water consumption”, “potential comparative toxic unit for ecosystems”,
“potential comparative toxic unit for humans – cancerogenic”, “Potential comparative toxic unit for humans - not cancerogenic”,
“potential soil quality index”. The results of this environmental impact indicator shall be used with care as the uncertainties on these
results are high as there is limited experience with the indicator.
References
Standards Regulation (EC) No 1907/2006 of the European
Parliament and of the Council on the Registration, Evaluation,
EN 15804 Authorisation and Restriction of Chemicals (REACH).
EN 15804:2012+A2:2019+AC:2021, Sustainability of
construction works — Environmental Product Declarations — GaBi
Core rules for the product category of construction products. Sphera Solutions GmbH
Gabi Software System and Database for Life Cycle
ISO 14025 Engineering 1992-2020
EN ISO 14025:2011, Environmental labels and declarations — Version 10.0.0.71, University of Stuttgart
Type III environmental declarations — Principles and Leinfelden-Echterdingen
procedures.
GaBi ts documentation
Further References GaBi life cycle inventory data documentation (https://www.gabi-
software.com/support/gabi/gabidatabase-
IBU 2021 2020-lci-documentation/).
Institut Bauen und Umwelt e.V.: General Instructions for the
EPD programme of Institut Bauen und Umwelt e.V., Version LCA-tool dormakaba
2.0, Berlin: Institut Bauen und Umwelt e.V., 2021 LCA-tool, IBU-DOR-202104-LT1-EN. Developed by Sphera
www.ibu-epd.com Solutions GmbH
EN 1154 PCR Part A
EN 1154-2003; Building hardware - Controlled door closing PCR – Part A: Calculation Rules for the Life Cycle Assessment
devices - Requirements and test methods. and Requirements on the Project Re-port according to EN
15804+A2:2019, Version 1.0, 2020, Institut Bauen und Umwelt
EN 1634-1 e.V., www.ibu-epd.com.
EN 1634-1:2018; Fire resistance and smoke control tests for
door and shutter assemblies, openable windows and elements PCR Part B
of building hardware - Part 1: Fire resistance test for door and PCR – Part B: Requirements on the EPD for Building Hardware
shutter assemblies and openable windows. product, version 08/2021, Institut Bauen und Umwelt e.V.,
www.ibu-epd.com.
REACH Regulation 1907/2006/EC
5 Environmental Product Declaration - dormakaba - TS 90 Impulse
Publisher
Institut Bauen und Umwelt e.V. +49 (0)30 3087748- 0
Hegelplatz 1 info@ibu-epd.com
10117 Berlin www.ibu-epd.com
Germany
Programme holder
Institut Bauen und Umwelt e.V. +49 (0)30 3087748- 0
Hegelplatz 1 info@ibu-epd.com
10117 Berlin www.ibu-epd.com
Germany
Author of the Life Cycle Assessment
Sphera Solutions GmbH +49 711 341817-0
Hauptstraße 111- 113 info@sphera.com
70771 Leinfelden-Echterdingen www.sphera.com
Germany
Owner of the Declaration
dormakaba International Holding GmbH +49 2333 793-0
DORMA Platz 1 info.de@dormakaba.com
58256 Ennepetal www.dormakaba.com
Germany
6 Environmental Product Declaration - dormakaba - TS 90 Impulse
