ENVIRONMENTAL PRODUCT DECLARATION
as per ISO 14025 and EN 15804+A1
Owner of the Declaration Troldtekt A/S
Programme holder Institut Bauen und Umwelt e.V. (IBU)
Publisher Institut Bauen und Umwelt e.V. (IBU)
Declaration number EPD-TRO-20220044-ICA1-EN
Issue date 07.04.2022
Valid to 06.04.2027
Acoustic panels - unpainted
Troldtekt A2 25 mm Natural Grey
based on FUTURECEM
www.ibu-epd.com | https://epd-online.com
Umwelt Produktdeklaration Name des Herstellers – Name des Produkts
1. General Information
Troldtekt A/S Troldtekt A2 25 mm Natural Grey
based on FUTURECEM - unpainted
Programme holder Owner of the declaration
IBU – Institut Bauen und Umwelt e.V. Troldtekt A/S
Panoramastr. 1 Sletvej 2 A
10178 Berlin 8310 Tranbjerg
Germany Denmark
Declaration number Declared product / declared unit
EPD-TRO-20220044-ICA1-EN Acoustic panel "A2 Natural Grey FUTURECEM" - 1 m2,
25 mm thickness - unpainted
This declaration is based on the product Scope:
category rules: This declaration represents the production, supply,
Wood cement - Mineral-bonded wooden composites, mounting, use, dismantling and disposal of 1 m2 (25
01.2019 mm thickness) of grey composite cement-bonded
(PCR checked and approved by the SVR) wood wool acoustic panel "A2 Natural Grey
FUTURECEM", produced by Troldtekt A/S, with a
reference service life of 50 years. The production
Issue date
facility is located in Jutland, Denmark. Three scenarios
07.04.2022
represent its use in indoor conditions in Denmark,
Sweden and Germany.
Valid to
06.04.2027
The owner of the declaration shall be liable for the
underlying information and evidence; the IBU shall not
be liable with respect to manufacturer information, life
cycle assessment data and evidences.
The EPD was created according to the specifications
of EN 15804+A1. In the following, the standard will be
simplified as EN 15804.
Verification
The standard EN 15804 serves as the core PCR
Independent verification of the declaration and data
according to ISO 14025:2010
Dipl. Ing. Hans Peters internally x externally
(chairman of Institut Bauen und Umwelt e.V.)
Dr. Alexander Röder Ms Jane Anderson
(Managing Director Institut Bauen und Umwelt e.V.)) (Independent verifier)
2. Product
2.1 Product description/Product definition For the application and use, the respective national
Troldtekt A2 Natural Grey FUTURECEM acoustic provisions apply.
panels are some of the leading and preferred solutions
for creating a good indoor sound environment. They 2.2 Application
are sold in various thicknesses (20-35 mm) and The panels are installed on the ceilings and walls in
dimensions (width: 600 mm, lengths: 600/1200/2400 offices, businesses, schools, institutions, cultural sites,
mm or width: 625 mm, lengths: 625/1250/2500 sports centres, swimming pools and private homes.
mm). The panels can be unpainted or painted in a wide
variety of colours. 2.3 Technical Data
The table below indicates the technical specifications
For the placing on the market of the product in the of the panels in accordance with EN 13168, the
European Union/European Free Trade Association standard for cement-bonded wood wool and double-
(EU/EFTA) (with the exception of Switzerland) layer panels with cement-bonded wood wool, and EN
Regulation (EU) No. 305/2011 applies. The product 13964, the standard for suspended ceilings.
needs a declaration of performance taking into
consideration EN 13964:2014, Suspended ceilings.
Requirements and test methods, and the CE-marking.
2 Environmental Product Declaration Troldtekt A/S – Troldtekt 25mm A2 Natural Grey FUTURECEM - unpainted
29 %. The wood is then shredded to produce wool.
The wood wool is mixed together with Portland
composite cement, water, and additives. The mixture is
cast and cured using a heat press and dried with a
biomass-fired oven. The cast panel is milled to remove
Technical specifications of the product covered in any material in excess and cut edges. After
this EPD approximately 4 weeks of curing, the panel can be
Name Value Unit painted before being stored on a pallet and packaged
Gross density 520 kg/m3 to be transported to central distribution warehouses.
Grammage 13.00 kg/m2
Thermal conductivity acc. to EN 2.7 Environment and health during
0.076 W/(mK)
13168:2012+A1:2015 manufacturing
Water vapour diffusion resistance Troldtekt is following its working environment closely.
- -
factor acc. to DIN 4108-4 Both the physical working environment and sickness
Sound absorption coefficient (only absence are closely monitored. It is an ongoing
with reference to the - % process involving both leaders and factory workers.
corresponding component design)
Light reflection (measured by 2.8 Product processing/Installation
DELTA Light and Optics 26.3 - 70.8 % Installation instructions are available here:
Reaction to fire A2/s1/d0 https://www.troldtekt.com/Installation
2.9 Packaging
The product is packaged with polyethylene plastic film
Performance data of the product in accordance with
and cardboard. The packaging material can be easily
the declaration of performance with respect to its
sorted and treated in dedicated waste recycling
essential characteristics according to EN
channels. The packaged product is delivered on a
13168:2012+A1:2015, Thermal insulation products for
returnable wood pallet.
buildings. Factory made wood wool (WW) products.
Specification and EN 13964:2014, Suspended ceilings.
Requirements and test methods.
2.10 Condition of use
Conditions of use are detailed
2.4 Delivery status
here: https://www.troldtekt.com/Installation/Use_and_
The panel is usually distributed in length of 600,
maintenance
1200 or 2400 mm by 600 mm width or in length of 625,
1250 or 2500 mm by 625 mm width. It comes in
2.11 Environment and health during use
three thicknesses: 20, 25 and 35 mm. Additionally,
Environmental and ecotoxicity risks from exposure to
several density ranges are available: Coarse, Fine,
Troldtekt panel products during use have been
Ultra-Fine and Extreme-Fine causing different
assessed and found eligible to the following
densities (388-428 kg/m3). The panels are normally
certification schemes:
delivered in packs of 80 units on pallets.
 Finnish M1 classification
2.5 Base materials/Ancillary materials  Danish Indoor Climate
The composition of the finished product is a mix of  Cradle to Cradle
limestone (19.3 %), wood wool (23.5 %), Portland
composite cement (54.4 %), water (0.6 %), as well as
These certificates can be accessed
water glass (1.0 %) and accelerator (1.3 %). The
here: https://www.troldtekt.com/Web-
composition is at dry basis at the factory gate, as most
tools/Downloads/Certificates-and-tests
of the water has evaporated during drying, but water
remains bound to the wood fibre and cement paste
2.12 Reference service life
(hydrated cement).
The technical service life of the panel is superior to 50
years. This EPD refers to the service lifetime indicated
This product/article/at least one partial article contains
by the BBSR table for the material 353.311 of type
substances listed in the candidate list (date:
“Holzbekleidungen: Holz, Holzwerkstoff und
17.01.2022) exceeding 0.1 percentage by mass: No
Mehrschichtleichtbauplatten”.
This product/article/at least one partial article contains
Because the panel is used in a building, in this EPD its
other CMR substances in categories 1A or 1B which
reference service life is limited by the expected service
are not on the candidate list, exceeding 0.1 percentage
life of the building, which is commonly accepted as 50
by mass: No
years, at least as LCA timeframe.
Biocide products were added to this construction
There is no influence of the ageing of the material on
product or it has been treated with biocide products
its technical performance.
(this then concerns a treated product as defined by the
(EU) Ordinance on Biocide Products No. 528/2012):
2.13 Extraordinary effects
No
Fire
2.6 Manufacture
Information on the fire performance according to EN
Norway spruce logs from local forests (with a moisture
13168.
content of about 65-70 %) are received and the bark is
removed. The wood is stored for approximately six
Fire protection
months until the moisture content in the wood drops to
Name Value
3 Environmental Product Declaration Troldtekt A/S – Troldtekt 25mm A2 Natural Grey FUTURECEM - unpainted
Building material class A2
Burning droplets d0 2.15 Disposal
Smoke gas development s1 The product may be composted, thermally treated with
energy recovery, or landfilled.
Water
No information on the product performance under the European Waste Code: 10 13 11 (wastes from
unforeseeable influence of water is available. cement-based composite materials)
Mechanical destruction Painted panels must be incinerated at end-of-life.
No information on the product performance under
unforeseeable mechanical destruction is available. Additional information on disposal
options: https://www.troldtekt.com/environment-and-
2.14 Re-use phase csr/product-life-cycle/recycling/
Currently, Troldtekt panels undergo thermal treatment
with energy recovery. Composting is also possible. 2.16 Further information
For additional information on technical specifications,
Additional information on recycling you may consult the Declaration Of
options: https://www.troldtekt.com/~/media/Files/Info% Performance: https://www.troldtekt.com/Web-
20sheets/English/Troldtekt_Recycling%20instructions tools/Downloads/DoPs
%20pdf.pdf
3. LCA: Calculation rules
3.1 Declared Unit
The functional unit is 1 m2 of acoustic panel, in 25 mm 3.6 Data quality
thickness, corresponding to 13.00 kg of material with Statistical representativeness
unpainted finish, mounted on the ceiling, with a The statistical representativeness of the product
reference service life of 50 years. system is very good. The input and output data
samples used to build inventories are based on the
Declared unit entirety of the annual production of panels in 2020 and
Name Value Unit is verified by a third party. Such representativeness is
Declared unit 1 m2 also valid for the production of Portland composite
Gross density 520 kg/m3 cement (FUTURECEM), whose EPD was published in
Grammage 13 kg/m2 2019 and audited in 2021. The EPD for the paint used
Layer thickness 0.025 m was published in 2018.
Temporal, geographical and technological
representativeness
3.2 System boundary All data strictly related to the cement production is
Cradle to grave technologically, temporally, and geographically
representative. The cement production data is less
3.3 Estimates and assumptions than 5 years old. The data used to model the
Assumptions are described occasionally throughout foreground inventory of acoustic panels dates from the
the section "LCA: Calculation rules". production year of 2020. As for secondary data, some
of the ecoinvent datasets are less than 3 years old.
3.4 Cut-off criteria
The cut-off criterion is applied according to EN 3.7 Period under review
15804 Section 6.3.5 and PCR part A Section 5.6. The primary data concerned with the manufacture (A1-
All inputs and outputs for which data are available are A3) relates to the production year 2020 and the data
included in the LCA model. Data gaps are filled with are based on the volumes produced on an annual
conservative assumptions from average data (when basis.
available) or with generic data and are documented
accordingly. 3.8 Allocation
The following product flows have been omitted Allocation of production data to the multiple produced
according to the 1 % cut-off rule: types of panels (with the same functional unit) is
 Wooden pallet to transport the product performed based on the rules provided in EN 15804.
Sub-processes associated to painting have especially
 Capital infrastructure (factory)
been allocated to the painted panels. Data such as
 Allocation of burden from wood logging to
waste generation and packaging have been allocated
residual wood fractions to the entire production volume of panels in Troldtekt.
The only case of co-produced outputs is associated to
wood logging. However, the environmental load is
evenly distributed over all its co-products, such as
3.5 Background data
logs, energy wood, and bark.
Two types of data source are used as secondary data:
 Product-specific EPDs for the manufacture
3.9 Comparability
and supply of Portland composite cement and
Basically, a comparison or an evaluation of EPD data
water-based paint
is only possible if all the data sets to be compared
 Database ecoinvent v.3.6 cut-off were created according to EN 15804 and the building
4 Environmental Product Declaration Troldtekt A/S – Troldtekt 25mm A2 Natural Grey FUTURECEM - unpainted
context, respectively the product-specific
characteristics of performance, are taken into account.
The used background database is ecoinvent v.3.6 cut-
off
4. LCA: Scenarios and additional technical information
Manufacture (A1-A3) empty runs)
Gross density of products
520 kg/m3
Data transported
Primary data is third-party verified and based on the Capacity utilisation volume factor 1 -
production year 2020, within the facilities of Troldtekt
A/S in Jutland (Denmark).
End-of-waste state and use of by-products
For all processes supplying a residual material/waste Installation into the building (A5)
that originates the end-of-life phase of a product to the Name Value Unit
product system to be used as input, the polluter-pay Electricity consumption 0.060 kWh
principle “100:0” is used. Some wooden by-products Material loss (plastic film) 0.007 kg
generated during manufacture in Troldtekt end up as Material loss (cardboard) 0.032 kg
soil improvers externally (reaching end-of-waste state),
and thus their biogenic carbon leaves Troldtekt's
Use phase (B1)
system boundary.
Prior to distribution and during the use phase (B1), the
carbonation of the cement contained in the panel,
Wind-certified electricity
during use, is accounted for. Based on laboratory
All the electricity used to produce the panels in Module
measurement, the panel will absorb up to 140 grams of
A3 originates from Danish wind power, for which a
carbon dioxide per kilogram of cement. Normalized to
certificate ensures the origin. It originates from a 1-3
the reference flow, this corresponds to an uptake of
MW offshore wind turbine, with transformation,
approximately 0.7 kilograms of carbon dioxide by the
transmission and distribution losses and is modelled
end of the service lifetime, including the uptake in A3.
correspondingly.
Maintenance (B2)
Carbon balance
As the panel does not require any maintenance except
Biogenic: Absorption of biogenic CO by the purchased
2 for the occasional dusting, no maintenance module
wood has been considered in A1. Some of it is
(B2) is considered.
released again during production in A3, some ends up
sequestered in soil, while the majority of the remaining
biogenic CO , 6.16 kg, is retained in the finished Name Value Unit
2
product and emitted during end-of-life incineration in
Repair, replacement, refurbishment (B3, B4, B5)
C4.
As the technical service life of the panel is superior to
Fossil: Absorption of some fossil CO , originating from
2 the assumed service life of the building (50 years), no
the calcination of limestone during cement production,
repair (B3), replacement (B4) or refurbishment (B5)
happens when the cement is mixed with water in A3. A
steps are considered.
majority is absorbed during the use phase B1, and all
the absorbed fossil CO is finally emitted during end-
2
of-life incineration in C4. Name Value Unit
Distribution to site (A4) and mounting (A5) Replacement (B4) / Refurbishment (B5)
To consider the main geographical variants of the life Name Value Unit
cycle of Troldtekt A2 Natural Grey FUTURECEM
panels, three scenarios are developed, where the Information about reference service life is detailed in
product is supplied, mounted, used and discarded in 2.12.
Aarhus (Denmark), Hamburg (Germany) and Malmö
(Sweden). An additional 50 km from the local Reference service life
warehouse to construction site is assumed. Name Value Unit
Reference service life (according to
50 a
ISO 15686-1, -2, -7 and -8)
Transport to the building site (A4) Life Span (according to BBSR) 50 a
Name Value Unit Life Span according to the
75 a
Litres of fuel 26.8 l/100km manufacturer
Transport distance to Denmark 160 km
Transport distance to Germany 370 km Operational energy use (B6) and Operational water
Transport distance to Sweden 394 km use (B7)
Transport distance from Name Value Unit
warehouse to local construction Water consumption - m3
50 km
sites in Electricity consumption - kWh
Denmark/Germany/Sweden Other energy carriers - MJ
Capacity utilisation (including 85 % Equipment output - kW
5 Environmental Product Declaration Troldtekt A/S – Troldtekt 25mm A2 Natural Grey FUTURECEM - unpainted
End of life (C1-C4)
Name Value Unit
Electricity use (for un-mounting) 0.060 kWh
Transport (to material sorting
50 km
facility)
Collected as mixed construction
13.00 kg
waste
Energy recovery 3.02 kg
Energy recovery efficiency 10 %
Energy recovered 6.15 MJ
The panel is un-mounted at the end of its reference
service life and driven to the regional waste
incineration plant. Energy is recovered from the wood
part of the panel at 10 % efficiency.
Reuse, recovery and/or recycling potentials (D),
relevant scenario information
Name Value Unit
Electricity 1.46 MJ
Heat 4.69 MJ
The energy substituted from incineration of the panel's
wood component in C4 is considered to be a split of
the Danish electricity grid mix (for electricity) and
natural gas (for heat).
Details on possible disposal routes
Aalborg Portland cement factory utilizes dust and
offcuts from the Troldtekt factory as a raw material in
new cement, i.e. in the technical circle. During
incineration in the cement kiln, the wood content in the
cement-bonded wood wool panels replaces fossil
fuels, while the cement ends up as a raw material in
new cement, replacing virgin raw materials and heavy
fossil fuels, thereby avoiding a significant amount of
CO emissions. This scheme of wood wool waste as a
2
raw material can be scaled for construction site and
demolition waste. It will be gradually rolled out to all of
Denmark in the period 2021-2023. Once Denmark has
documented economic and environmental benefits to
be gained by including wood wool waste in the
production of new cement rather than going to waste
incineration or landfill, dialogue with municipalities and
local cement producers in the primary markets of
Troldtekt is initiated to facilitate similar schemes
regionally or nationally.
6 Environmental Product Declaration Troldtekt A/S – Troldtekt 25mm A2 Natural Grey FUTURECEM - unpainted
5. LCA: Results
Note: Global Warming Potential (GWP) indicator includes CO of both biogenic and fossil origin.
2
Also, GWP results for Troldtekt A2 Natural Grey FUTURECEM (unpainted) for other delivery scenarios in
respectively Germany and Sweden, are 2.57E-1 kg CO and 2.72E-1 kg CO .
2 2
DESCRIPTION OF THE SYSTEM BOUNDARY (X = INCLUDED IN LCA; MND = MODULE NOT DECLARED;
MNR = MODULE NOT RELEVANT)
BENEFITS AND
CONSTRUCTI LOADS
PRODUCT STAGE ON PROCESS USE STAGE END OF LIFE STAGE BEYOND THE
STAGE SYSTEM
BOUNDARIES
7 Environmental Product Declaration Troldtekt A/S – Troldtekt 25mm A2 Natural Grey FUTURECEM - unpainted
lairetam
waR
ylppus tropsnarT
gnirutcafunaM
eht
morf
tropsnarT
etis
eht
ot
etag
ylbmessA esU
ecnanetniaM
riapeR
tnemecalpeR tnemhsibrufeR
ygrene
lanoitarepO esu
retaw
lanoitarepO esu
noitcurtsnoc-eD
noitilomed tropsnarT
gnissecorp
etsaW
lasopsiD -esueR -yrevoceR -gnilcyceR laitnetop
A1 A2 A3 A4 A5 B1 B2 B3 B4 B5 B6 B7 C1 C2 C3 C4 D
X X X X X X MND MNR MNR MNR MND MND X X MND X X
RESULTS OF THE LCA - ENVIRONMENTAL IMPACT according to EN 15804+A1: 1 m2 A2 Natural Grey
FUTURECEM, 25 mm, unpainted, delivered and used in Denmark
Parameter Unit A1-A3 A4 A5 B1 C1 C2 C4 D
GWP [kg CO2-Eq.] -1.41E-1 1.29E-1 8.76E-2 -5.24E-1 6.50E-4 1.05E-1 6.86E+0 -8.04E-1
ODP [kg CFC11-Eq.] 2.30E-7 2.35E-8 1.64E-9 0.00E+0 2.81E-10 1.92E-8 5.40E-9 -4.44E-8
AP [kg SO2-Eq.] 1.37E-2 2.60E-4 5.90E-5 0.00E+0 1.59E-6 2.13E-4 4.46E-4 -1.67E-3
EP [kg (PO4)3--Eq.] 5.69E-3 5.35E-5 1.03E-4 0.00E+0 8.86E-7 4.37E-5 1.94E-4 -1.24E-3
POCP [kg ethene-Eq.] 7.63E-4 1.71E-5 2.58E-6 0.00E+0 8.88E-8 1.40E-5 3.49E-5 -9.59E-5
ADPE [kg Sb-Eq.] 6.05E-5 3.51E-6 2.09E-7 0.00E+0 1.82E-8 2.87E-6 5.88E-7 -2.16E-6
ADPF [MJ] 4.07E+1 1.96E+0 3.70E-1 0.00E+0 4.20E-2 1.60E+0 5.39E-1 -1.13E+1
GWP = Global warming potential; ODP = Depletion potential of the stratospheric ozone layer; AP = Acidification potential of land and water; EP =
Caption Eutrophication potential; POCP = Formation potential of tropospheric ozone photochemical oxidants; ADPE = Abiotic depletion potential for non-
fossil resources; ADPF = Abiotic depletion potential for fossil resources
RESULTS OF THE LCA - INDICATORS TO DESCRIBE RESOURCE USE according to EN 15804+A1: 1 m2
A2 Natural Grey FUTURECEM, 25 mm, unpainted, delivered and used in Denmark
Parameter Unit A1-A3 A4 A5 B1 C1 C2 C4 D
PERE [MJ] 5.99E+1 2.76E-2 1.60E-1 0.00E+0 3.91E-2 2.26E-2 7.12E+0 -5.26E+0
PERM [MJ] 6.21E+1 0.00E+0 0.00E+0 0.00E+0 0.00E+0 0.00E+0 0.00E+0 0.00E+0
PERT [MJ] 1.22E+2 2.76E-2 1.60E-1 0.00E+0 3.91E-2 2.26E-2 7.12E+0 -5.26E+0
PENRE [MJ] 5.19E+1 1.97E+0 4.58E-1 0.00E+0 4.31E-2 1.61E+0 5.63E-1 -1.42E+1
PENRM [MJ] 0.00E+0 0.00E+0 0.00E+0 0.00E+0 0.00E+0 0.00E+0 0.00E+0 0.00E+0
PENRT [MJ] 5.19E+1 1.97E+0 4.58E-1 0.00E+0 4.31E-2 1.61E+0 5.63E-1 -1.42E+1
SM [kg] 2.26E+0 0.00E+0 3.10E-2 0.00E+0 0.00E+0 0.00E+0 0.00E+0 0.00E+0
RSF [MJ] 5.13E+0 0.00E+0 0.00E+0 0.00E+0 0.00E+0 0.00E+0 0.00E+0 0.00E+0
NRSF [MJ] 5.73E+0 0.00E+0 0.00E+0 0.00E+0 0.00E+0 0.00E+0 0.00E+0 0.00E+0
FW [m³] 3.50E-2 3.35E-4 1.30E-4 0.00E+0 1.19E-5 2.73E-4 2.37E-4 -1.54E-3
PERE = Use of renewable primary energy excluding renewable primary energy resources used as raw materials; PERM = Use of
renewable primary energy resources used as raw materials; PERT = Total use of renewable primary energy resources; PENRE = Use of
non-renewable primary energy excluding non-renewable primary energy resources used as raw materials; PENRM = Use of non-
Caption
renewable primary energy resources used as raw materials; PENRT = Total use of non-renewable primary energy resources; SM = Use
of secondary material; RSF = Use of renewable secondary fuels; NRSF = Use of non-renewable secondary fuels; FW = Use of net fresh
water
RESULTS OF THE LCA – WASTE CATEGORIES AND OUTPUT FLOWS according to EN 15804+A1:
1 m2 A2 Natural Grey FUTURECEM, 25 mm, unpainted, delivered and used in Denmark
Parameter Unit A1-A3 A4 A5 B1 C1 C2 C4 D
HWD [kg] 5.91E-2 1.99E-3 1.51E-3 0.00E+0 5.40E-5 1.62E-3 1.25E-3 -4.91E-2
NHWD [kg] 1.91E+0 1.37E-1 1.15E-1 0.00E+0 1.12E-3 1.12E-1 5.23E-2 -1.67E+0
RWD [kg] 9.00E-5 1.34E-5 2.54E-6 0.00E+0 5.78E-7 1.10E-5 4.20E-6 -2.04E-5
CRU [kg] 0.00E+0 0.00E+0 0.00E+0 0.00E+0 0.00E+0 0.00E+0 0.00E+0 0.00E+0
MFR [kg] 1.05E-2 0.00E+0 0.00E+0 0.00E+0 0.00E+0 0.00E+0 0.00E+0 0.00E+0
MER [kg] 4.86E-3 0.00E+0 0.00E+0 0.00E+0 0.00E+0 0.00E+0 0.00E+0 0.00E+0
EEE [MJ] 0.00E+0 0.00E+0 0.00E+0 0.00E+0 0.00E+0 0.00E+0 1.46E+0 0.00E+0
EET [MJ] 0.00E+0 0.00E+0 0.00E+0 0.00E+0 0.00E+0 0.00E+0 4.69E+0 0.00E+0
HWD = Hazardous waste disposed; NHWD = Non-hazardous waste disposed; RWD = Radioactive waste disposed; CRU = Components
Caption for re-use; MFR = Materials for recycling; MER = Materials for energy recovery; EEE = Exported electrical energy; EET = Exported
thermal energy
6. LCA: Interpretation
The estimated impact results are only relative by the acquisition and use of cement and wood in the
statements that do not indicate the end points of the foreground processes. Global Warming Potential net
impact categories, exceeding threshold values, safety emissions share is much larger in C4 than in A1-A3
margins or risks. (see why in chart (2)), while other impact categories in
module D, in general, are avoided in the waste system
Two charts are presented: (1) with the standard owing to the incineration of end-of-life panels and
lifecycle impact categories displaying the share of substitution of natural gas and Danish electricity mix.
impacts across all lifecycle stages, and (2) displaying C4 also slightly follows emissions of compounds
the total carbon balance of the Troldekt product's associated to other impact categories. A relatively
lifecycle system. inefficient transportation of end-of-life panels to waste
incineration causes emissions in especially Abiotic
Impacts from the A1-A3 modules are dominant in the depletion of non-fossil resources, Depletion of
life cycle of the Troldtekt A2 Natural Grey stratospheric ozone, and Photochemical ozone
FUTURECEM panel products. This is primarily caused formation.
The embodied emissions associated to the raw A1-A3 and some fossil CO taken up in A1-A3 and B1
2
materials (primarily cement) are the main cause of is re-emitted in C4. CO emissions ocuring in the
2-eq
impacts, especially in terms of net Global Warming remaining modules are negligible.
Potential, with 4.85 kg CO for cement followed by
2-eq
minor impacts from additives. In general, direct The amount of wood stored in the product refers to a
emissions from the Troldtekt production site are negative contribution to Global Warming Potential,
relatively small. Abiotic depletion of fossil resources reducing the share of Global Warming Potential in A1-
appears from the burden of producing cement using A3. This is due to the sequestration of biogenic carbon
fossil raw material such as limestone and to a large of wood during tree growth. The sequestered carbon
extent fossil fuels. In terms of carbon balance, biogenic does not contribute to global warming as long as it is
CO in A1-A3 offsets nearly all the fossil CO stored in the biomass.
2 2
emissions in A1-A3. All biogenic CO sequestered in
2
Summary
8 Environmental Product Declaration Troldtekt A/S – Troldtekt 25mm A2 Natural Grey FUTURECEM - unpainted
Within the cradle to grave, the following aspects have
been identified as major contributors, mainly in the The clinker (cement) production is the most critical
categories Global Warming Potential and Abiotic process of the Troldtekt product system, but
depletion of fossil resources: inaccuracies around the amount used will not
invalidate the present conclusions.
 Emissions from the clinker production from
material Notably, by introducing more up-to-date LCA datasets
for the grey cement applied, or introducing cements
 Emissions from the clinker production from
with less carbon footprint into production could lead to
fuel
significant reductions of especially the Global Warming
 Substituted emissions from end of life Potential indicator.
incineration
7. Requisite evidence
Technological Institute under DANAK accreditation
7.1 Testing of substances used 392. Report no. MAIC-2019-1418. Reporting of
A detailed assessment of substances used was measured concentrations in toluene equivalents
conducted by a DAkkS-accredited laboratory, based according to EN 16516. This test is the basis for the
on a sample (prepared according to EN 15443), Finish M1 Material certificate as well as the Danish
available in the Test Report 2018P216294, using Indoor Climate labelling certificate.
inductively coupled plasma mass spectrometry (EN
16171) and X-ray fluorescence (EN 15309), for the AgBB overview of results (28 days [µg/m³])
following: Name Value Unit
 Heavy metals (cadmium, mercury, etc.) TVOC (C6 - C16) 12 μg/m3
 and other elements Sum SVOC (C16 - C22) 0 - 5 μg/m3
VOC without NIK 0 - 5 μg/m3
Carcinogenic Substances 1 μg/m3
7.2 Leaching
No leaching measurement was conducted according
AgBB overview of results (3 days [µg/m³])
to EN 717-1.
Name Value Unit
TVOC (C6 - C16) - μg/m3
Sum SVOC (C16 - C22) - μg/m3
7.3 VOC emissions
R (dimensionless) - -
Testing for VOC emissions has been conducted in
VOC without NIK - μg/m3
accordance with EN ISO 16000-6. Analysis of the air
Carcinogenic Substances - μg/m3
sampled on Tenax was performed at the Danish
8. References
Standards
DIN EN ISO 14025
DIN EN ISO 14025:2011, Environmental labels and
AgBB declarations – Type III environmental
AgBB, Ausschuss zur gesundheitlichen Bewertung von declarations – Principles and procedures, German and
Bauprodukten (Committee for Health-related English versions EN ISO 14025:2011
Evaluation of Building Products)
EN 13168
BBSR EN 13168:2012+A1:2015, Thermal insulation products
BBSR, Bundesinstitut für Bau-, Stadt- und for buildings. Factory made wood wool (WW) products.
Raumforschung (Federal Institute for Research on Specification
Building, Urban Affairs and Spatial Development).
BBSR table: EN 13964
https://www.nachhaltigesbauen.de/fileadmin/pdf/baust EN 13964:2014, Suspended ceilings. Requirements
off_gebauededaten/BNB_Nutzungsdauern_von_Bautei and test methods
len_2017-02-24.pdf
EN 15309
DIN 4108-4 EN 15309:2007, Characterization of waste and soil.
DIN 4108-4:2017-03, Thermal insulation and energy Determination of elemental composition by X-ray
economy in buildings - Part 4: Hygrothermal design fluorescence
values
EN 15443
DIN 52612-2 EN 15443:2011, Solid recovered fuels. Methods for the
DIN 52612-2, Testing of thermal insulating materials; preparation of the laboratory sample
determination of thermal conductivity by means of the
guarded hot plate apparatus; conversion of the EN 15804
measured values for building applications. 1 June 1984
9 Environmental Product Declaration Troldtekt A/S – Troldtekt 25mm A2 Natural Grey FUTURECEM - unpainted
EN 15804:2012, EN 15804:2012+A1 2013,
Sustainability of construction works – Environmental Product Category Rule A
Product Declarations – Core rules for the product Product Category Rule A, IBU, 2019, Part A,
category of construction products. Calculation Rules for the Life Cycle Assessment and
Requirements on the Project Report. v.1.8. IBU, 2019.
EN 16171
EN 16171:2016, Sludge, treated biowaste and soil. Product Category Rule B
Determination of elements using inductively coupled Product Category Rule B, IBU, 2019, Part B,
plasma mass spectrometry (ICP-MS) Requirements on the EPD for Wood cement - Mineral-
bonded wooden composites. v.1.7. IBU, 2019.
EN 16449
EN 16449:2014, EN 16449:2014, Wood and wood- Regulation (EU) No. 305/2011
based products - Calculation of the biogenic carbon
content of wood and conversion to carbon dioxide
Further References
EN 16516
EN 16516:2017+A1:2020, Construction products: General Programme Instructions, IBU 2021
Assessment of release of dangerous substances. General Instructions for the EPD programme of Institut
Determination of emissions into indoor air Bauen und Umwelt e.V. Version 2.0, Berlin: Institut
Bauen und Umwelt e.V., 2021. www.ibu-epd.com
EN 717-1
EN 717-1:2004, Wood-based Panels – Determination Software/database
of Formaldehyde Release – Formaldehyde emission OneClick LCA software, Pre-verified EPD tool,
by the chamber method Bionova: https://www.oneclicklca.com/
European Waste Code: 10 13 11 Database: Ecoinvent v.3.6. cut-off (2019)
(wastes from cement-based composite materials) https://ecoinvent.org/the-ecoinvent-database/
ISO 16000-6
ISO 16000-6:2011, Indoor air - Part 6: Determination of
volatile organic compounds in indoor and test chamber
air by active sampling on Tenax TA sorbent, thermal
desorption and gas chromatography using MS or MS-
FID
10 Environmental Product Declaration Troldtekt A/S – Troldtekt 25mm A2 Natural Grey FUTURECEM - unpainted
Publisher
Institut Bauen und Umwelt e.V. Tel +49 (0)30 3087748- 0
Panoramastr. 1 Fax +49 (0)30 3087748- 29
10178 Berlin Mail info@ibu-epd.com
Germany Web www.ibu-epd.com
Programme holder
Institut Bauen und Umwelt e.V. Tel +49 (0)30 - 3087748- 0
Panoramastr 1 Fax +49 (0)30 – 3087748 - 29
10178 Berlin Mail info@ibu-epd.com
Germany Web www.ibu-epd.com
Author of the Life Cycle
Assessment Tel 98777223
Aalborg Portland Fax 80815733
Rørdalsvej 44 Mail
92200 Aalborg Ø stefan.e.danielsson@cementirhol
Denmark ding.it
Web www.aalborgportland.dk
Owner of the Declaration
Troldtekt A/S Tel +45 8747 8100
Sletvej 2A Fax +45 8747 8111
8310 Tranbjerg J Mail sales@troldtekt.dk
Denmark Web https://www.troldtekt.com
