ENVIRONMENTAL PRODUCT DECLARATION
as per ISO 14025 and EN 15804+A2
Owner of the Declaration Etex Building Performance International
Publisher Institut Bauen und Umwelt e.V. (IBU)
Programme holder Institut Bauen und Umwelt e.V. (IBU)
Declaration number EPD-ETE-20230253-IBA2-EN
Issue date 08.04.2024
Valid to 24.09.2028
Promatect-MST®, Promatect-MT®, Promarine 450T®, Promarine
640T®, Supalux M1®, Vermiculux T®, Promatect-MLT®, Promasil®
1100 Super and Promasil® 1000L
PROMAT
www.ibu-epd.com | https://epd-online.com
1. General Information
PROMAT Promatect-MST®, Promatect-MT®, Promarine
450T®, Promarine 640T®, Supalux M1®,
Vermiculux T®, Promatect-MLT®, Promasil® 1100
Super and Promasil® 1000L
Programme holder Owner of the declaration
IBU – Institut Bauen und Umwelt e.V. Etex Building Performance International
Hegelplatz 1 Rue Marcel Demonque 500
10117 Berlin 84915 Avignon Cedex 9
Germany France
Declaration number Declared product / declared unit
EPD-ETE-20230253-IBA2-EN 1 m2 of Promatect-MST® with a thickness of 40 mm
This declaration is based on the product category rules: Scope:
Calcium silicate insulating materials, 01.08.2021 This EPD is representative and relevant for Promatect-MST®, Promarine
(PCR checked and approved by the SVR) 450T®, Promarine 640T®, Supalux M1®, Promatect-MT®, Vermiculux T®,
Promatect-MLT®, Promasil® 1100 Super and Promasil® 1000L boards
produced by ETEX in Tisselt (Belgium) and installed in Europe. The data
Issue date describing the direct inputs and outputs of the foreground processes are
representative for ETEX production in Tisselt, Belgium, and taken from the
08.04.2024
period of one year between October 2020 and September 2021.
The results in this EPD are based on Promatect-MST®. In the LCA
Valid to
background report the representativeness of Promatect-MST® has been
24.09.2028 checked by comparing the LCA results of Promatect-MST® with the LCA
results of the other products included in the scope of the EPD.
The owner of the declaration shall be liable for the underlying information
and evidence; the IBU shall not be liable with respect to manufacturer
information, life cycle assessment data and evidences.
The EPD was created according to the specifications of EN 15804+A2. In
the following, the standard will be simplified as EN 15804.
Verification
The standard EN 15804 serves as the core PCR
Dipl.-Ing. Hans Peters
Independent verification of the declaration and data according to ISO
(Chairman of Institut Bauen und Umwelt e.V.)
14025:2011
internally X externally
Florian Pronold Vito D'Incognito,
(Managing Director Institut Bauen und Umwelt e.V.) (Independent verifier)
Environmental Product Declaration - PROMAT - Promatect-MST®, Promatect-MT®, Promarine 450T®, Promarine 640T®, Supalux M1®, Vermiculux T®, Promatect-
1 MLT®, Promasil® 1100 Super and Promasil® 1000L
2. Product
Name Value Unit
2.1 Product description/Product definition
Gross density EN12467 300 - 750 kg/m3
Promatect-MST®, Promarine 450T®, Promarine 640T®,
Supalux M1®, Promatect-MT®, Vermiculux T®, Promatect- Flexural strength EN 12467 >2.0 N/mm2
MLT®, Promasil® 1100 Super and Promasil® 1000L. Thermal conductivity at 20°C, Hot Wire 0.138 -
W/(mK)
This EPD describes the life cycle analysis of different Promat MEthod 0.250
products for fire protection. The product ranges under Compressive strength 2 - 18 N/mm2
consideration are the cement-bounded medium-density calcium
silicate fire protective boards. In detail, the investigated
Products according to the CPR based on an ETA:
products are 9 for this range, including Promatect MT®,
For the placing of the product on the market in the European
Promatect MST®, Promatect MLT®, Promarine 450T®,
Union/European Free Trade Association (EU/EFTA) (with the
Promarine 640T®, Supalux M1®, Vermiculux T®, Promasil®
exception of Switzerland) the Regulation (EU) No. 305/2011
1100 Super and Promasil® 1000L.
(CPR) applies. The product needs a declaration of performance
The boards are self-supporting, non-combustible, asbestos-free
taking into consideration ETA no. 22/0581: 2023-03-10,
and moisture-resistant calcium silicate fire protection boards for
PROMATECT-MST®. For the application and use the
a variety of applications. The products differentiate by individual
respective national provisions apply.
densities and the ratios of included raw materials to meet the
technical requirements of individual applications.
2.4 Delivery status
The function of these fire protective boards is generally equal
The products have a thickness of 12.7, 20, 25, 30, 40, 50 or 60.
being the provision of structural fire protection. This can be by
The length is 2500 mm.
covering walls, floorings, and ceilings in buildings, by covering
The width is 1200 mm.
structural steelwork or by constructing fire-resistant ducts and
same applications apply to Promarine boards within the Marine
The products are transported and delivered on a wooden pallet
sector.
and packed with cartons and PET straps.
Products according to the CPR based on an ETA: 2.5 Base materials/Ancillary materials
For the placing of the product on the market in the European
The main constituents of the product are silica (20-35 %),
Union/European Free Trade Association (EU/EFTA) (with the
cement (10-30 %), lime (10-30 %), cellulose fibres (1-10 %) and
exception of Switzerland) the Regulation (EU) No. 305/2011
other minerals (5-25 %).
(CPR) applies. The product needs a declaration of performance
taking into consideration ETA no. 22/0581: 2023-03-10,
This product/article/at least one partial article contains
PROMATECT-MST®. For the application and use the
substances listed in the candidate list (date: accesses
respective national provisions apply.
31/07/2023) exceeding 0.1 percentage by mass: no
2.2 Application
This product/article/at least one partial article contains other
Promatect-MST®, Supalux M1®, Promatect-MT®, Vermiculux
carcinogenic, mutagenic, reprotoxic (CMR) substances in
T®, Promatect-MLT® boards are versatile multi-purpose fire
categories 1A or 1B which are not on the candidate list,
protection boards, for multiple applications:
exceeding 0.1 percentage by mass: no
• FIRE-RATED ASSEMBLIES: Building and industrial
construction, among other things for fire dampers and Biocide products were added to this construction product or it
smoke extraction dampers, fire doors and metal profile has been treated with biocide products (this then concerns a
insulator treated product as defined by the (EU) Ordinance on Biocide
Products No. 528/2012): no
Promarine 450T®, Promarine 640T®
• A, B & C Class divisions
2.6 Manufacture
• Compartmentations
There is only one manufacturing plant of the declared products
• Linings
being the manufacturing plant in Tisselt (Belgium). The
• Non-combustible furniture
products are all produced on the same type of production line.
All raw materials, including previously made xonotlite slurries,
Promasil® 1100 Super and Promasil® 1000L
together with a balanced amount of water are mixed to form a
• Aluminium industry: anode baking furnace and
slurry, and shaped by a filter press to produce a wet board. It is
electrolysis cells
steam cured in an autoclave to form required calcium silicate
• Steel industry: smelting and heat treatment furnaces
minerals suitable for the end application. Final steps are the
• Glass industry: melting furnaces, heat treatment and
drying, cutting and sanding/finishing. During the cutting and
foming furnaces
finishing, scrap is produced which is partly recycled, both
• Ceramics industry: bogie hearth furnaces, kiln cars
internally and externally, and partly landfilled.
• Cement industry: heat exchangers and cyclone
separators 2.7 Environment and health during manufacturing
• Oil and gas industry: fired heaters pipe supports Environmental, occupational health, safety and quality
management at the Guangzhou plant are in accordance with
2.3 Technical Data
the following standards:
Constructional data · ISO 14001;2015
· ISO 9001;2015
· ISO 45001:2018
2.8 Product processing/Installation
Environmental Product Declaration - PROMAT - Promatect-MST®, Promatect-MT®, Promarine 450T®, Promarine 640T®, Supalux M1®, Vermiculux T®, Promatect-
2 MLT®, Promasil® 1100 Super and Promasil® 1000L
Not considered in the EPDs. Various installation scenarios exist Name Value
depending on the application.
Building material class A1
2.9 Packaging Burning droplets /
The products are transported and delivered on a wooden pallet Smoke gas development /
and packed with cartons and PET straps.
Water
2.10 Condition of use
Tests on the product performance including possible impacts on
B modules are not included. These products are designed for
the environment following the unforeseeable influence of water,
life and depending on the application in which the products are
e.g. flooding showed that no risks are expected to occur in
used there might be a need for
terms of environment and human health.
maintenance/repair/replacement of the application.
2.11 Environment and health during use Mechanical destruction
In case of mechanical destruction, no risks are expected to
Under normal conditions of use, the products do not cause any
occur in terms of environment and human health.
adverse health effects or release of volatile organic compounds
(VOCs) into indoor air. No environmental impact on water, air or 2.14 Re-use phase
soil is expected due to the extremely low metal release from the
Currently, the boards can be recycled as a replacement of filler
low maintenance requirements.
(e.g. secondary limestone fillers). In the EPD, both the 100 %
2.12 Reference service life recycling and 100 % landfill scenario have been calculated.
The RSL depends on the application. Under normal conditions 2.15 Disposal
of use, the product is supposed to remain its characteristics as
The waste number according to the European list 'Decision N°
long as the application lasts. For application in building a
2000/532/CE' is '17 09 00: other construction and demolition
reference service life of 60 years (i.e life time of the building)
wastes'.
could be declared.
2.16 Further information
2.13 Extraordinary effects
https://www.promat.com/en-ie/industry/products-
Fire
solutions/passive-fire-protection/board-products/promatect-mst/
Information on the fire performance according to EN 13501:1.
Fire protection
3. LCA: Calculation rules
3.1 Declared Unit 3.3 Estimates and assumptions
1 m2 of Promatect-MST® with a thickness of 40 mm. The results in this EPD are based on Promatect-MST®. In the
LCA background report the representativeness of Promatect-
Declared unit
MST® has been checked by comparing the LCA results of
Name Value Unit Promatect-MST® with the LCA results of the other products
Declared unit 1 m2 included in the scope of the EPD. This study showed that for
Gross density 750 kg/m3 most of the indicators Promatect-MST® can be considered the
most conservative of the product range in terms of
Grammage 30 kg/m2
environmental impact. Only Promarine 640 T® has a higher
Mass of the declared product 0.03 t environmental impact, but the variance is limited to 30 %, and
The results in this EPD are based on Promatect-MST®. In the less than 12 % for the three most relevant impact indicators,
LCA background report the representativeness of Promatect- according to the PEF single score (i.e. Climate change,
MST® has been checked by comparing the LCA results of Acidification and Resource use fossils).
Promatect-MST® with the LCA results of the other products
3.4 Cut-off criteria
included in the scope of the EPD.
The following processes are considered below cut-off according
to the rules as per the PCR, Part A:
Assuming a linear relationship between the thickness and the
mass/environmental impact of the board, the environmental • Packaging of raw materials, as the main raw materials
impact of a product can be considered to be proportional to the (i.e. largest amounts) come in bulk
thickness of the product, so products with another thickness • Ancillary materials for production
can be calculated by the below formula: • Infrastructure and land use of the factory
• Environmental impacts caused by the personnel of the
E=W*Eref/Wref production plants are not included in the LCA, e.g.
waste from the cafeteria and sanitary installations,
E=environmental impact of a product with density d and accidental pollution caused by human mistakes, or
thickness t environmental effects caused by commuter traffic.
W=d*t=weight of 1 m2 product with density d and thickness t Heating or cooling of the plants in order to ensure a
Eref=environmental impact of the reference product comfortable indoor climate for the personnel for
Wref=weight of 1 m2 reference product example is also neglected.
3.5 Background data
Ecoinvent 3.8 and Industry 2.0
3.2 System boundary
3.6 Data quality
Cradle-to-gate with options, including modules C2-C4 and D
Environmental Product Declaration - PROMAT - Promatect-MST®, Promatect-MT®, Promarine 450T®, Promarine 640T®, Supalux M1®, Vermiculux T®, Promatect-
3 MLT®, Promasil® 1100 Super and Promasil® 1000L
Company-specific data concern the data about the production available, as the data per production step or product line could
of Promatect-MST®. All required data about the production be extracted. In this case, the data have been allocated to the
process have been delivered to Enperas by ETEX. declared unit using the annual production volume of that
product in m2.5 (i.e. 1 m2 with a thickness of 5 mm is the
The composed datasets for this project are representative and reference unit in ETEX's factory). The last step was to
relevant for Promatect-MST®, Promarine 450T®, Promarine recalculate the amount to the declared unit by multiplying with
640T®, Supalux M1®, Promatect-MT®, Vermiculux T®, the mass ratio between 1 m2.5 and 1 m2 with the thickness
Promatect-MLT®, Promasil® 1100 Super and Promasil® 1000L declared in the EPD. This approach has been used for all
produced by ETEX in Tisselt, Belgium. inputs and outputs, except for water use/discharge and
production waste-externally recycled.
3.7 Period under review
For the water use/discharge only facility-level data were
The data collected by ETEX are based on data from the period
available. These have been allocated to the individual product
of one year between October 2020 and September 2021.
using the annual production volume in kg. For the production
waste-externally recycled, facility-level data were available for
3.8 Geographic Representativeness
all the declared products together with two other Promat
Land or region, in which the declared product system is
products of the Tisselt plant. These have been allocated to the
manufactured, used or handled at the end of the product´s
individual product using the annual production volume in kg.
lifespan: Europe
3.10 Comparability
3.9 Allocation Basically, a comparison or an evaluation of EPD data is only
No co-products are produced. possible if all the data sets to be compared were created
No secondary raw materials are used. according to EN 15804 and the building context, respectively
At ETEX's plant in Tisselt, different types of calcium silicate the product-specific characteristics of performance, are taken
boards are produced. into account.
For most of the production data, product specific data is Ecoinvent 3.8 and Industry 2.0
4. LCA: Scenarios and additional technical information
the incoming waste).
Characteristic product properties of biogenic carbon 3. the remaining powder (<100µm) will be used as filler
The Promat boards contain biogenic carbon in the form of replacing limestone in cement applications
cellulose (assumed 0,44 kg C/kg cellulose). Also, its packaging Name ValueUnit
contains biogenic carbon in the form of cartons (assumed 0,44
Collected as mixed construction waste 30 kg
kg C/kg carton) and wooden pallets (assumed 0,45 kg C/kg
Recycling Scenario 1 (cellulose content is
wood). 30 kg
incinerated)
Information on describing the biogenic carbon content at
Landfilling Scenario 2 30 kg
factory gate
Reuse, recovery and/or recycling potentials (D), relevant
Name ValueUnit
scenario information
kg
Biogenic carbon content in product 0.667 In module D, the benefits and loads beyond the system
C
boundaries are quantified. For recycling, it concerns both the
Biogenic carbon content in accompanying 0.509 kg loads of the recycling processes after the end-of-waste and the
packaging C benefits of the avoided virgin materials, when the recycled
components are used for other purposes. In case of
incineration, it concerns the benefits from the avoided
production of energy grace to energy recovery.
End of life (C1-C4)
In the EPD, both 100 % recycling and 100 % landfill scenario
Benefits of recycling the product in limestone production have
have been calculated. Recycling consists in
been included in module D (avoided impact of limestone
1. milling/crushing the boards production and energy recovery from incineration of cellulose),
2. sieving out the fibres which will be incinerated and used together with some minor benefits and loads due to recycling
as an energy source (to heat up the machine and dry and energy recovery of the packaging.
Environmental Product Declaration - PROMAT - Promatect-MST®, Promatect-MT®, Promarine 450T®, Promarine 640T®, Supalux M1®, Vermiculux T®, Promatect-
4 MLT®, Promasil® 1100 Super and Promasil® 1000L
5. LCA: Results
Note that module A5 only includes waste treatment of the packaging of the final product. Installation itself has not been included, as a
wide variety exists depending on the application.
Note that both 100 % recycling (scenario 1) and 100 % landfill (scenario 2) scenarios have been calculated.
DESCRIPTION OF THE SYSTEM BOUNDARY (X = INCLUDED IN LCA; ND = MODULE OR INDICATOR NOT DECLARED; MNR =
MODULE NOT RELEVANT)
Benefits and
Construction loads beyond
Product stage Use stage End of life stage
process stage the system
boundaries
la ire ta m w a Ry lp p u s tro p s n a rT g n iru tc a fu n a M e h t m o rf tro p s n a rTe tis e h t o t e ta g y lb m e s s A e s U e c n a n e tn ia M ria p e R tn e m e c a lp e R tn e m h s ib ru fe R y g re n e la n o ita re p Oe s u re ta w la n o ita re p Oe s u n o itc u rts n o c -e Dn o itilo m e d tro p s n a rT g n is s e c o rp e ts a W la s o p s iD -e s u e R-y re v o c e R-g n ilc y c e Rla itn e to p
A1 A2 A3 A4 A5 B1 B2 B3 B4 B5 B6 B7 C1 C2 C3 C4 D
X X X MND X MND MND MNR MNR MNR MND MND MND X X X X
RESULTS OF THE LCA - ENVIRONMENTAL IMPACT according to EN 15804+A2: 1 m^2 Promatect-MST®, Promarine 450T®,
Promarine 640T®, Supalux M1®, Promatect-MT®, Vermiculux T®, Promatect-MLT®
Parameter Unit A1-A3 A5 C2/1 C2/2 C3/1 C3/2 C4/1 C4/2 D/1 D/2
GWP-total kg CO 2 eq 2.81E+01 1.64E+00 2.85E-01 2.51E-01 2.63E+00 0 0 2.44E+00 -1.23E+00 -6.7E-01
GWP-fossil kg CO 2 eq 3.26E+01 3.62E-02 2.85E-01 2.51E-01 3.67E-01 0 0 1.82E-01 -7.13E-01 -1.57E-01
GWP-
biogenic kg CO 2 eq -4.58E+00 1.6E+00 1.02E-04 8.98E-05 2.26E+00 0 0 2.25E+00 -5.13E-01 -5.12E-01
GWP-luluc kg CO 2 eq 7.86E-03 1.38E-05 1.14E-04 1E-04 7.95E-04 0 0 1.34E-04 -1.25E-03 -7.03E-04
ODP kg CFC11 eq 3.59E-06 7.07E-09 6.61E-08 5.82E-08 2.8E-08 0 0 6.74E-08 -8.22E-08 -1.85E-08
AP mol H+ eq 8.83E-02 2.13E-04 8.1E-04 7.13E-04 2.45E-03 0 0 1.61E-03 -3.62E-03 -6.6E-04
EP-
kg P eq 2.43E-04 3.9E-07 2.03E-06 1.79E-06 3.57E-05 0 0 5.58E-06 -3.49E-05 -1.09E-05
freshwater
EP-marine kg N eq 2.44E-02 8.84E-05 1.61E-04 1.42E-04 5.28E-04 0 0 5.48E-04 -9.07E-04 -1.6E-04
EP-terrestrial mol N eq 2.6E-01 8.77E-04 1.79E-03 1.58E-03 5.96E-03 0 0 6.05E-03 -1.17E-02 -1.76E-03
kg NMVOC
POCP 7.49E-02 2.59E-04 6.89E-04 6.07E-04 1.59E-03 0 0 1.72E-03 -2.92E-03 -6.13E-04
eq
ADPE kg Sb eq 2.04E-05 8.33E-08 7.72E-07 6.8E-07 8.1E-07 0 0 4.32E-07 -1.76E-06 -4.06E-07
ADPF MJ 3.64E+02 4.98E-01 4.32E+00 3.81E+00 7.39E+00 0 0 5.2E+00 -1.3E+01 -2.87E+00
m3 world eq
WDP 7.96E-01 2.77E-03 1.32E-02 1.16E-02 9.53E-02 0 0 2.43E-02 -1.17E-01 -5.54E-02
deprived
GWP = Global warming potential; ODP = Depletion potential of the stratospheric ozone layer; AP = Acidification potential of land and water; EP =
Eutrophication potential; POCP = Formation potential of tropospheric ozone photochemical oxidants; ADPE = Abiotic depletion potential for non-fossil
resources; ADPF = Abiotic depletion potential for fossil resources; WDP = Water (user) deprivation potential)
RESULTS OF THE LCA - INDICATORS TO DESCRIBE RESOURCE USE according to EN 15804+A2: 1 m^2 Promatect-MST®,
Promarine 450T®, Promarine 640T®, Supalux M1®, Promatect-MT®, Vermiculux T®, Promatect-MLT®
Parameter Unit A1-A3 A5 C2/1 C2/2 C3/1 C3/2 C4/1 C4/2 D/1 D/2
PERE MJ 6.19E+01 4.47E+00 6.08E-02 5.35E-02 1.08E+00 0 0 2.68E-01 0 0
PERM MJ 4.11E+01 -9.26E+00 0 0 -1.97E+01 0 0 0 2.45E+01 4.81E+00
PERT MJ 1.03E+02 -4.8E+00 6.08E-02 5.35E-02 -1.84E+01 0 0 2.68E-01 2.45E+01 4.81E+00
PENRE MJ 4.02E+02 5.7E-01 4.35E+00 3.83E+00 7.51E+00 0 0 5.33E+00 0 0
PENRM MJ 1.18E-01 -7.23E-02 0 0 0 0 0 0 3.42E-02 3.42E-02
PENRT MJ 4.02E+02 4.76E-01 4.35E+00 3.83E+00 8.76E+00 0 0 5.33E+00 3.42E-02 3.42E-02
SM kg 5.8E-02 0 0 0 0 0 0 0 0 0
RSF MJ 0 0 0 0 0 0 0 0 0 0
NRSF MJ 0 0 0 0 0 0 0 0 0 0
FW m3 2.78E-01 2.99E-04 3.18E-04 2.8E-04 6.21E-03 0 0 5.59E-03 -6.1E-03 -1.87E-03
PERE = Use of renewable primary energy excluding renewable primary energy resources used as raw materials; PERM = Use of renewable primary
energy resources used as raw materials; PERT = Total use of renewable primary energy resources; PENRE = Use of non-renewable primary energy
excluding non-renewable primary energy resources used as raw materials; PENRM = Use of non-renewable primary energy resources used as raw
materials; PENRT = Total use of non-renewable primary energy resources; SM = Use of secondary material; RSF = Use of renewable secondary fuels;
NRSF = Use of non-renewable secondary fuels; FW = Use of net fresh water
RESULTS OF THE LCA – WASTE CATEGORIES AND OUTPUT FLOWS according to EN 15804+A2:
1 m^2 Promatect-MST®, Promarine 450T®, Promarine 640T®, Supalux M1®, Promatect-MT®, Vermiculux T®, Promatect-MLT®
Parameter Unit A1-A3 A5 C2/1 C2/2 C3/1 C3/2 C4/1 C4/2 D/1 D/2
HWD kg 4.77E-04 1.15E-06 1.13E-05 9.94E-06 4.03E-06 0 0 5.7E-06 -1.57E-05 -3.94E-06
NHWD kg 5.22E+00 4.07E-01 2.26E-01 1.99E-01 5.05E-02 0 0 3E+01 -4.06E-02 -1.94E-02
Environmental Product Declaration - PROMAT - Promatect-MST®, Promatect-MT®, Promarine 450T®, Promarine 640T®, Supalux M1®, Vermiculux T®, Promatect-
5 MLT®, Promasil® 1100 Super and Promasil® 1000L
RWD kg 7.32E-04 3.22E-06 2.92E-05 2.57E-05 5.3E-05 0 0 3.55E-05 -5.37E-05 -1.24E-05
CRU kg 0 0 0 0 0 0 0 0 0 0
MFR kg 0 3.4E-01 0 0 3E+01 0 0 0 0 0
MER kg 0 0 0 0 0 0 0 0 0 0
EEE MJ 0 4.49E-01 0 0 0 0 0 0 0 0
EET MJ 0 8.97E-01 0 0 0 0 0 0 0 0
HWD = Hazardous waste disposed; NHWD = Non-hazardous waste disposed; RWD = Radioactive waste disposed; CRU = Components for re-use;
MFR = Materials for recycling; MER = Materials for energy recovery; EEE = Exported electrical energy; EET = Exported thermal energy
RESULTS OF THE LCA – additional impact categories according to EN 15804+A2-optional:
1 m^2 Promatect-MST®, Promarine 450T®, Promarine 640T®, Supalux M1®, Promatect-MT®, Vermiculux T®, Promatect-MLT®
Parameter Unit A1-A3 A5 C2/1 C2/2 C3/1 C3/2 C4/1 C4/2 D/1 D/2
Disease
PM 4.38E-07 3.65E-09 2.29E-08 2.02E-08 1.17E-08 0 0 3.11E-08 -4.04E-08 -1.38E-08
incidence
IR kBq U235 eq 5.48E-01 2.23E-03 1.88E-02 1.65E-02 6.39E-02 0 0 2.66E-02 -5.91E-02 -1.34E-02
ETP-fw CTUe 2.35E+02 4.46E-01 3.39E+00 2.99E+00 7.27E+00 0 0 2.99E+00 -6.85E+01 -1.82E+00
HTP-c CTUh 6.11E-09 1.08E-10 1.09E-10 9.61E-11 6.01E-10 0 0 8.66E-11 -2.15E-10 -7.56E-11
HTP-nc CTUh 1.42E-07 6.58E-10 3.43E-09 3.02E-09 6.51E-09 0 0 1.75E-09 -5.53E-09 -1.78E-09
SQP SQP 4.55E+02 4.92E-01 3.01E+00 2.65E+00 1.61E+00 0 0 9.8E+00 -5.93E+01 -5.79E+01
PM = Potential incidence of disease due to PM emissions; IR = Potential Human exposure efficiency relative to U235; ETP-fw = Potential comparative
Toxic Unit for ecosystems; HTP-c = Potential comparative Toxic Unit for humans (cancerogenic); HTP-nc = Potential comparative Toxic Unit for humans
(not cancerogenic); SQP = Potential soil quality index
Disclaimer 1 – for the indicator “Potential Human exposure efficiency relative to U235”. This impact category deals mainly with the
eventual impact of low-dose ionizing radiation on human health of the nuclear fuel cycle. It does not consider effects due to possible
nuclear accidents, occupational exposure or radioactive waste disposal in underground facilities. Potential ionizing radiation from the
soil, radon and from some construction materials is also not measured by this indicator.
Disclaimer 2 – for the indicators “abiotic depletion potential for non-fossil resources”, “abiotic depletion potential for fossil resources”,
“water (user) deprivation potential, deprivation-weighted water consumption”, “potential comparative toxic unit for ecosystems”,
“potential comparative toxic unit for humans – cancerogenic”, “Potential comparative toxic unit for humans - not cancerogenic”,
“potential soil quality index”. The results of this environmental impact indicator shall be used with care as the uncertainties on these
results are high as there is limited experience with the indicator.
6. LCA: Interpretation
The environmental profile shows the contribution of the various highest contribution on all impact categories. Also, the transport
steps in the life cycle, per environmental impact category. For of the raw materials to the factory is significant for several
the declared products produced in Belgium, the manufacturing impact indicators.
stage and raw materials used in the formulation mix have the
7. Requisite evidence
8. References
Standards ISO 9001
EN 12467 ISO 9001:2015: Quality management systems — Requirements
EN 12467:2012+A2:2018, Fibre-cement flat sheets. Product ISO 14001
specification and test methods
ISO 14001:2015: Environmental management systems —
EN 13501-1 Requirements with guidance for use
DIN EN 13501-1:2019-05: Fire classification of ISO 14025
constructionproducts and building elements - Part 1:
Classification usingdata from reaction to fire tests EN ISO 14025:2011, Environmental labels and declarations —
Type III environmental declarations — Principles and
EN 15804 procedures.
EN 15804:2012+A2:2019+AC:2021, Sustainability of ISO 14040
construction works — Environmental Product Declarations —
Core rules for the product category of construction products. ISO 14040:2006: Environmental management – Life cycle
assessment – Principles andframework.
EN 16757
ISO 14044
EN 16757:2017, Sustainability of construction works–
Environmental product declarations – Product Category Rules ISO 14044:2006: Environmental management – Life cycle
for concrete and concrete elements assessment – Requirements and guidelines.
Environmental Product Declaration - PROMAT - Promatect-MST®, Promatect-MT®, Promarine 450T®, Promarine 640T®, Supalux M1®, Vermiculux T®, Promatect-
6 MLT®, Promasil® 1100 Super and Promasil® 1000L
ISO 45001 LCA database as integrated in SimaPro 9.3.0.3.
ISO 45001:2018:Occupational health and safety management Ordinance on Biocide Products No. 528/2012
systems Requirements with guidance for use
Biocidal Products Regulation, BPR, Regulation (EU) 528/2012
Further references
PCR Part A
CPR
Calculation rules for the Life Cycle Assessment and
European Regulation N° 305/2011 (CPR) Requirements on the Background Report, Institut Bauen und
Umwelt e.V., www.bauumwelt.com.
ECHA candidate list
PCR Part B
Candidate List of substances of very high concern (SVHCs)
forauthorisation, last update 26.07.2022, European Institut Bauen und Umwelt e.V, Berlin (pub.): PCR Guidance-
ChemicalsAgency (ECHA), Helsinki, Finland Texts for Building-Related Products and Services From the
range of Environmental Product Declarations of Institute
Ecoinvent Construction and Environment e.V. (IBU) : Requirements on the
EPD for Calcium silicate insulating materials
Wernet, G., Bauer, C., Steubing, B., Reinhard, J., Moreno-Ruiz,
E., and Weidema, B., 2016. The ecoinvent database version 3 PEFCR
(part I): overview and methodology. The International Journal of
Life Cycle Assessment, [online] 21(9), pp.1218–1230. Available European commission (2018). Product Environmental Footprint
at:http://link.springer.com/10.1007/s11367-016-1087-8. Category Rules PEFCR Guidance, version 6.3.
Enperas Pré Consultants (2021)
Quadrant tool. 2023. Genk, Belgium SimaPro 9.2.0.1 [Computer Software]. Amersfoort, The
Netherlands.
European Waste Code
REACH
Commission of the European Communities, 2010, Guidance on
classification of waste according to EWC-Stat categories Regulation (EC) No 1907/2006 of the European Parliament and
of the Council of 18 December 2006 concerning the
IBU Registration, Evaluation, Authorisation and Restriction of
Chemicals (REACH), June 2017
IBU 2021. Institut Bauen und Umwelt e.V.: General Instructions
for the EPD programme of Institut Bauen und Umwelt e.V.,
Version 2.0, Berlin: Institut Bauen und Umwelt e.V., 2021 The literature referred to in the Environmental Product
www.ibu-epd.com Declaration must be listed in full.Standards already fully quoted
in the EPD do not need to be listed here again.
Industry 2.0 The current version of PCR Part A and PCR Part B of the PCR
document on which they are based must be referenced.
Industry 2.0 (from PlasticsEurope, worldsteel and ERASM).
Environmental Product Declaration - PROMAT - Promatect-MST®, Promatect-MT®, Promarine 450T®, Promarine 640T®, Supalux M1®, Vermiculux T®, Promatect-
7 MLT®, Promasil® 1100 Super and Promasil® 1000L
Publisher
Institut Bauen und Umwelt e.V. +49 (0)30 3087748- 0
Hegelplatz 1 info@ibu-epd.com
10117 Berlin www.ibu-epd.com
Germany
Programme holder
Institut Bauen und Umwelt e.V. +49 (0)30 3087748- 0
Hegelplatz 1 info@ibu-epd.com
10117 Berlin www.ibu-epd.com
Germany
Author of the Life Cycle Assessment
Enperas +32 3 376 00 19
Thorpark 8300 info@enperas.com
3600 Genk https://www.enperas.com/en/
Belgium
Owner of the Declaration
Etex Building Performance International +32 2 778 12 11
Rue Marcel Demonque 500 info@etexgroup.com
84915 Avignon Cedex 9 www.etexgroup.com
France
Environmental Product Declaration - PROMAT - Promatect-MST®, Promatect-MT®, Promarine 450T®, Promarine 640T®, Supalux M1®, Vermiculux T®, Promatect-
8 MLT®, Promasil® 1100 Super and Promasil® 1000L
