ENVIRONMENTAL PRODUCT DECLARATION
as per ISO 14025 and EN 15804+A2
Owner of the Declaration Adolf Würth GmbH & Co. KG
Publisher Institut Bauen und Umwelt e.V. (IBU)
Programme holder Institut Bauen und Umwelt e.V. (IBU)
Declaration number EPD-AWU-20230269-IBD1-EN
Issue date 12.09.2023
Valid to 12.09.2027
flexen®PE
Adolf Würth GmbH & Co. KG
www.ibu-epd.com | https://epd-online.com
1. General Information
Adolf Würth GmbH & Co. KG flexen®PE
Programme holder Owner of the declaration
IBU – Institut Bauen und Umwelt e.V. Adolf Würth GmbH & Co. KG
Hegelplatz 1 Reinhold-Würth-Str. 12-17
10117 Berlin 74653 Künzelsau
Germany Germany
Declaration number Declared product / declared unit
EPD-AWU-20230269-IBD1-EN flexen® PE
This declaration is based on the product category rules: Scope:
Insulating materials made of foam plastics, 01.08.2021 Product line flexen® PE Thermal insulation products for building
(PCR checked and approved by the SVR) equipment and industrial insulations made of polythene [BSJ1] foam
(PEF) according to EN14313, describing the specific environmental
performance of the product produced in Belgium at the site of Eynatten
Issue date The owner of the declaration shall be liable for the underlying information
and evidence; the IBU shall not be liable with respect to manufacturer
12.09.2023
information, life cycle assessment data and evidences.
The EPD was created according to the specifications of EN 15804+A2. In
Valid to
the following, the standard will be simplified as EN 15804.
12.09.2027
Verification
The standard EN 15804 serves as the core PCR
Independent verification of the declaration and data according to ISO
14025:2011
internally X externally
Dipl.-Ing. Hans Peters
(Chairman of Institut Bauen und Umwelt e.V.)
Florian Pronold Vito D'Incognito,
(Managing Director Institut Bauen und Umwelt e.V.) (Independent verifier)
1 Environmental Product Declaration - Adolf Würth GmbH & Co. KG - flexen®PE
2. Product
inside diameter. They
2.1 Product description/Product definition are delivered in lengths of 2 m packed in cardboard. (More
flexen® PE Polyethylene foams have many environmental information on ranges and dimensions on WÜRTH
benefits, having a low density (average 24.3 kg/m³), few raw (wuerth.de).)
materials are required for the manufacture of an article and the
environmental 2.5 Base materials/Ancillary materials
impact of their transport is lower than similar articles of
Base materials
higher density performing the same function. Furthermore, the
flexen® PE are flexible insulation materials containing recycled
flexen® PE are fully recyclable.
PE, which is produced
For the placing on the market of the product in the European
using a mixture of up to seven basic component materials. The
Union/European Free Trade Association (EU/EFTA )(with the
following table displays an average weighted of different
exception of Switzerland) - Thermal Insulation products for
elements of the formulation, and this for the complete flexen®
building equipment and industrial installations cf. PCR. Factory
PE product range. The following table displays the different
made polyethylene foam (PEF) and the CE-marking. For the
elements of the formulation for flexen® PE. This is in
application
accordance with the PCR Part B: Requirements on the EPD for
and use the respective national provisions apply
Insulating materials made of foam plastics and ISO14025. This
2.2 Application product contains substances listed in the candidate list (date:
08.07.2021) exceeding 0.1
The function of flexen® PE is to insure the insulation of heating
percentage by mass: No.
and sanitary installations for a reference service life (RSL) of 50
This product contains other carcinogenic, mutagenic, reprotoxic
years.
(CMR) substances in categories 1A or 1B, which are not on the
This duration is based on the frequency of replacement of
candidate list, exceeding 0.1 percentage by mass: No.
sanitary and heating piping in buildings. Although the insulation
Biocide products were added to this construction product or it
pipes are still effective after 50 years, it is assumed that when
has been treated with biocide products (this then concerns a
replacing the piping, the insulation flexen® PE is not reused
treated product as defined by the (EU) Ordinance on Biocide
and
Products 528/2012) : No
is recycled. 50 years is the minimum Reference Service Life
recommended in EN 16783 Name Value Unit
LDPE 36.50 %
2.3 Technical Data
Flame Retardant 5.70 %
The technical specifications of the products within the scope of
LLDPE 18.51 %
the EPD shall be listed, including the reference to the test
methods/test standards for each specification. Internally recycled PE 25.10 %
Pigment 3.76 %
For products with CE marking, the technical specifications must Volume stabilizer 2.00 %
be specified in accordance with information in the declaration of
Blowing Agent 8.43 %
performance. The properties relevant to the product should be
specified in the table below. If no information is given for Low Density Polyethylen (LDPE), internally recycled PE and
properties, an explanation must be given in the background fillers are the main components of the product and are
report to the EPD as to why the property is not relevant to the responsible for the characteristics and
product. performance of the product The blowing agent causes the
expansion during manufacturing. The flame retardant ensures
the fire resistance and conformity with fire protection
Constructional data
regulations (see section 2.13). According the European
Performance data of the product in accordance with
Chemicals Regulation REACH manufacturers, importers and
the Declaration of Performance with respect to its
downstream users must register their chemicals and are
Essential Characteristics according to EN 14313 apply. Further
responsible for their safe use. Adolf Würth GmbH & Co. KG
data:
uses exclusively verifiably registered and approved substances
Name Value Unit in its production. flexen® PE do not contain Substances of Very
Gross density 24.3 kg/m3 High Concern (SVHC). Antimony trioxide and halogenated
flame retardants are used.
Thermal conductivity 0.036 - 0.048 W/(mK)
Reaction To Fire Acc. to EN 13501-1 Bl-s1d0 ; Cl-
-
depending on the thickness s1d0 2.6 Manufacture
Max Service Temperature Acc. To EN The manufacturing process consists of a continuous extrusion.
100 °C
14707 Solid pellets of thermoplastic resin are fed into a melting zone
Min Service Temperature 0 °C in which the resin is melted, to form a flowable thermoplastic
water absorption Acc. to EN 13472 WS005 - mass. The thermoplastic mass is then metered to a mixing
zone where it is
traces quantities of water-soluble ions Cl < 10 – F < 4
- thoroughly mixed with a blowing agent under pressure.
and pH-value Acc. to EN 13468 - pH 6,8
The mixture of thermoplastic resin and blowing agent is then
forced through a die, which imparts a shape to the
thermoplastic mass, into a zone of lower pressure (i.e.
2.4 Delivery status
atmospheric pressure). The blowing agent expands to form the
The flexen® PE product is a closed-cell polyethylene foam, cells of the foam and the thermoplastic foam is cooled through
containing recycled PE, insulation tube designed for an inline water cooler. At the end of the inline cooler the profiles
applications in heating and sanitary installations. The flexen® are cut to the required dimensions.
PE range extends from 5 to 25 mm thick and from 12 to 114mm
2 Environmental Product Declaration - Adolf Würth GmbH & Co. KG - flexen®PE
Quality assurance : The function of flexen® PE is to ensure the insulation of heating
The manufacture is certified ISO 9001 for quality management. and sanitary installations for a reference service life (RSL) of 50
The product corresponds to the product standard EN 14313 years. This duration is based on the frequency of replacement
and has a Declaration of of sanitary
Performance according to the DOP no. and heating piping in buildings. Although the insulation pipes
LE_0870609015_01_M_flexen_PE are still effective after 50 years, it is assumed that when
(see www.wuerth.de) replacing the piping, the insulation (flexen® PE ) is recycled. 50
years is the minimum Reference Service Life recommended in
2.7 Environment and health during manufacturing EN16783 "PCR for factory made thermal insulation products".
During all manufacturing steps the production follows all Description of the influences on the ageing of the product when
national guidelines and regulations. Solar panels are installed applied in accordance with the rules of technology.
on the roof of
the warehouse and in the field to reduce the requirement for
grid electricity. 2.13 Extraordinary effects
Fire
2.8 Product processing/Installation flexen® PE is classified as a combustible insulation material.
flexen® PE can be installed using basic tools (e.g. craft knives). Due to its material structure, flexen® PE does not contribute to
No special tools, nor specific protection is necessary. When an uncontrollable spread of fire under installation conditions
applying adhesives the information given in the relevant safety typical on a building site. The product is self-extinguishing
data sheets is reducing its contribution to any fire event. There is no possibility
to be heeded. Any glue and adhesive tapes used during the of the material
installation phase were not included in the LCA. self-igniting. flexen® PE does not propagate the fire horizontally
Recommendations on how to use the product are described in or vertically. The smoke development in case of fire is very low
the application manuals or videos. More details are listed on (class S1).
the Web Page WÜRTH (wuerth.de).
Fire protection
2.9 Packaging Name Value
flexen® PE products are packed in cardboard boxes and Building material class Bl/Cl
transported on reusable pallets. All packaging material can be Burning droplets d0
recycled. The pallets used to transport the products are taken
Smoke gas development s1
back or exchanged when the flexen® PE is delivered, so the
use of pallets is a closed loop economy.
Water
2.10 Condition of use flexen® PE is a closed cell foam and obtains the best water
During the use of the products for the purpose for absorption class WS005 according to the product standard.
which they are intended, there are no modifications
unless one of the effects listed in extraordinary impacts Mechanical destruction
occurs (see point 2.13). flexen® PE is chemically inert and does not present any
environmental or health risk if mechanically destructed. flexen®
2.11 Environment and health during use
PE is not UV resistant. The product is not recommended for
There are no particular effects on environmental and health outside applications without complementary UV protection
impacts during use related to the material composition of the
product. The 2.14 Re-use phase
flexen® PE products are used in a wide range of applications In principle, if removed carefully, flexen® PE can be reused on
across the building sector. The PEF foams fulfil the German, any other piping system of similar dimensions. Any material not
Belgian and French regulations regarding the emission of VOC suitable for reuse is fully recyclable.
with emissions far below the most stringent limit values. The
Eurofin Product Testing institute, at the request of the CEFEP 2.15 Disposal
(European group of PEF and FEF manufacturers) has made a The flexen® PE is fully recyclable and can be used as a direct
wide range of tests for different PEF products from different one-for-one substitute for virgin PE-LD granulates, with only
manufacturers. The insulation of heating pipes with flexen® PE minor additive additions. There is no chemical difference
allows a reduction of energy dispersion and of course CO between recycled PE and fossil fuel derived PE-LD, so using a
2
emissions during the full service life of the installation. The mix of sources does not change the recyclability of the product.
quantification of this in-use benefit is not within the scope of this
2.16 Further information
EPD, however, this could be calculated using an LCA for the
Additional information about flexen® PE can be found on the
complete pipe/insulation system, and has to be evaluated in the
web site www.wuerth.de Here specification clauses, data
frame of the LCA from the complete heating installation.
sheets and application manuals can be found.
2.12 Reference service life
3. LCA: Calculation rules
Declared unit
3.1 Declared Unit
The declared unit for insulating materials made of foam plastic
is 1 m³. The EPD will cover the whole flexen® PE range. The
insulating
sleeves in the flexen® PE range have a thickness ranging from
5 to 25mm and an inside diameter ranging from 12 to 114mm
The average reference density of flexen® PE is 24.3 kg/m³.
3 Environmental Product Declaration - Adolf Würth GmbH & Co. KG - flexen®PE
Name Value Unit Module C2:
Gross density 24.3 kg/m3 Transport at the end-of-life stage is modelled as a Euro Cargo
0-6 mix truck with diesel fuel. The average distance to either
Declared unit 1 m3
mechanical recycling, incineration or landfills is assumed to be
Declared unit - λ 100 km.
Value for 1 m divided Module C3:
Conversion factor from 1
section of the insulation pipe m The scenario that has been retained for
m³ to 1 linear meter
( m²) this Life Cycle Assessment is the 100% recycling
Gross Density volume for scenario.
1 kg 0.0412 m³ Module C4:
As flexen® PE is fully
Thermal Conductivity at
0.040 W/(mK) recyclable, the legislation is pushing more in this
40°C
direction and the overall pressure on plastic recycling
Thermal Conductivity λ : 0.040 W/mK at (40°C) is growing, the scenario with recycling is considered.
R-value- thickness- : 25 mm : +/- 3.5 (m²K/W) Module D:
depending on the pipe diameter. The flexen® PE is fully
recyclable and can be used as a direct one-for-one
substitute for virgin PE-LD granulates, with only minor
3.2 System boundary
additive additions.
The Data collection refers to the yearly production in 2021.
Module A1 to A3: 3.3 Estimates and assumptions
The LCA calculation covers the production of the raw materials, The LCA calculation is conducted using the Gabi ts - database.
transport of these to the plant, the mixing of raw materials Not all necessary LCIs are included in the database. Where
according to the respective recipes, manufacturing of the foam data were missing or were unavailable or where suppliers were
product and packaging for dispatch. All production takes place unable to provide complete information, proxy datasets have
exclusively in Eynatten, Belgium. been used.
Module A4: The environmental burden for the production of pigments, flame
The logistics department reported average figures for the retardants and volume stabilizers are approximated.
distribution of products - depending on the country the transport
distance varies. The biggest customers represent 85% of sales 3.4 Cut-off criteria
volumes in 2021, with the remainder supplied to Any glue and adhesive tapes used during the installation (A5)
a large set of smaller customers. have not been included as quantification of these materials is
Module A5: uncertain and their use by the various installers is too diverse,
Installation of flexen® PE products is done by hand and adhesives
requires no special equipment apart from a knife. The products and glues are not required in all/most cases, but may
can be be used for some applications. In this study no others cut-off
placed end to end and the remaining pieces can be reused. criteria have been applied and all elementary incoming
Some glue or tape could be used for the installation, as the processes as well
quantity of the product used depends on the final customer, he as all energy and water inputs and waste outputs have been
has to calculate the impact of what he used himself. The counted.
environmental
3.5 Background data
impact of this type of accessory is not counted in this study. The
calculations do not contain any installation waste. Cardboard as The software system for life cycle engineering GaBi
a packaging material is assumed to be recycled. As input 10 developed by thinkstep AG was used to perform
material cardboard made of waste paper is considered. Thus, this LCA. The GaBi LCI database GaBi 10 provides
the environmental burden of packaging materials are the life cycle inventory data for several of the raw and
considered already in A1-A3. The value of the environmental process materials obtained from the background
impact for A5 system. The most recent update of the database was
is declared as '0'. The choice made is : the final user has to in 2021.
calculate the impact of A5 himself in the function of his own
3.6 Data quality
case, by accounting for the extra amount of product needed
All the foreground data requiring such energy or raw material
during installation.
coming from production, were verified and cross-checked
Module B1-B7:
before being included in the model. Most of the life cycle
Once installed the flexen® PE product requires no maintenance
inventories for the basic materials are included in the GaBi 10
and no repair. It will be dismantled when the sanitary pipe is
software. For electrical and thermal energy Belgium-specific
replaced. For this reason, there are not expected to be any
grid mixes and Belgium-specific supply for natural gas were
impacts in B1 to B7 assuming correct specification and
considered.
installation. Step B1 is not considered in this LCA, although the
insulation of the piping contributes to a significant reduction of
3.7 Period under review
CO emissions from the heating or cooling equipment, this
2 The production data for the year 2021 were used for the
is not taken into account in this LCA. It should,
realization of this study
however, be taken into account in the calculation of the
environmental impacts of the complete heating and 3.8 Geographic Representativeness
cooling systems or of the complete building. Land or region, in which the declared product system is
Module C1: manufactured, used or handled at the end of the product´s
As for the installation of the product, the disassembly is done lifespan: Germany
manually and does not require any specific equipment.
Disassembly is generally carried out at the same time as the
replacement or removal of sanitary pipes. Consequently, there 3.9 Allocation
are no impacts associated with C1.
4 Environmental Product Declaration - Adolf Würth GmbH & Co. KG - flexen®PE
There is no co-product or by-product generated during the no special equipment apart from a knife. Installation off-cut is
production of Adolf Würth GmbH & Co. KG products. Due to the not considered in this calculations. Any glue and adhesive
lack of specific data per production line and product, the energy tapes used during the installation phase were not included in
has been allocated per overall produced volume of insulation the LCA
foam.
Production waste 3.10 Comparability
Most of the production waste from the process (machine start, Basically, a comparison or an evaluation of EPD data is only
end of production, non-conforming products, etc.) is recycled possible if all the data sets to be compared were created
internally in order to be reused in the manufacturing process. according to EN 15804 and the building context, respectively
These impacts the product-specific characteristics of performance, are taken
are accounted for in A1-A3. into account.
Installation and End-of-Life waste The used background database has to be mentioned.
Installation of the foam products is done by hand and requires
4. LCA: Scenarios and additional technical information
A5 is not declared including the disposal of the packaging
Characteristic product properties of biogenic carbon material on the construction site, the amounts of packaging
The biogenic carbon content quantifies the amount of biogenic materials included in the LCA calculations must be declared as
carbon in a construction product leaving the factory gate, and it technical scenario information for Module A5.
shall be separately declared for the product and for any
accompanying packaging.
If the total mass of biogenic carbon containing materials is less
Transport to the building site (A4)
than 5 % of the total mass of the product and accompanying
packaging, the declaration of biogenic carbon content may be Name Value Unit
omitted. The mass of packaging containing biogenic carbon Litres of fuel 0.045 l/100km
shall always be declared. Transport distance 488 km
Capacity utilisation (including empty runs) 10 %
Note: 1 kg of biogenic carbon is equivalent to 44/12 kg of CO2.
Gross density of products transported 24.3 kg/m3
Information on describing the biogenic Carbon Content at
factory gate In case a reference service life according to applicable ISO
standards is declared then the assumptions and in-use
Name ValueUnit
conditions underlying the determined RSL shall be declared. In
kg
Biogenic carbon content in product - addition, it shall be stated that the RSL applies to the reference
C
conditions only.
Biogenic carbon content in accompanying kg
3.62
packaging C The same holds for a service life declared by the manufacturer.
Corresponding information related to in-use conditions needs
not be provided if a service life taken from the list of service life
The following technical scenario information is required for the
by BNB is declared.
declared modules and optional for non-declared modules.
Modules for which no information is declared can be deleted;
additional information can also be listed if necessary. Reference service life
Name Value Unit
The following technical information is a basis for the declared
Reference service life 50 a
modules or can be used for developing specific scenarios in the
context of a building assessment if modules are not declared End of life (C1-C4)
(MND).
Name Value Unit
Recycling 24.3 kg
5 Environmental Product Declaration - Adolf Würth GmbH & Co. KG - flexen®PE
5. LCA: Results
In Table 1 "Description of the system boundary", all declared modules shall be indicated with an "X"; all modules that are not declared
shall be indicated with "MND" (As default the modules B3, B4, B5 are marked as MNR – module not relevant). In the following tables,
columns can be deleted for modules that are not declared. Indicator values should be declared with three valid digits (eventually using
the exponential form (e.g. 1,23E-5 = 0,0000123). A uniform format should be used for all values of one indicator.
If several modules are not declared and therefore have been deleted from the table, the abbreviations for the indicators can be
replaced by the complete names, while the readability and clear arrangement should be maintained; the legends can then be deleted.
If due to relevant data gaps, an indicator cannot be declared in a robust way, then the abbreviation “IND” (indicator not declared)
should be used for this indicator.
• 0 - calculated value is 0
• 0 - value falls under the cut-off
• 0 - assumption which exclude any flows (e.g. exported
electricity A1-A3)
• IND – in cases where the inventory does not support
the methodological approach or the calculation of the
specific indicator IND shall be used.
If no reference service life is declared (see chapter 2.13 "Reference Service Life"), the LCA results of the modules B1-B2 and B6-B7
shall refer to a period of one year. This shall then be indicated as an explanatory text below the tables. In addition, the formula for the
quantification of such B-modules over the total life cycle shall be provided.
DESCRIPTION OF THE SYSTEM BOUNDARY (X = INCLUDED IN LCA; ND = MODULE OR INDICATOR NOT DECLARED; MNR =
MODULE NOT RELEVANT)
Benefits and
Construction loads beyond
Product stage Use stage End-of-life stage
process stage the system
boundaries
la ire ta m w a Ry lp p u s tro p s n a rT g n iru tc a fu n a M e h t m o rf tro p s n a rTe tis e h t o t e ta g y lb m e s s A e s U e c n a n e tn ia M ria p e R tn e m e c a lp e R tn e m h s ib ru fe R y g re n e la n o ita re p Oe s u re ta w la n o ita re p Oe s u n o itc u rts n o c -e Dn o itilo m e d tro p s n a rT g n is s e c o rp e ts a W la s o p s iD -e s u e R-y re v o c e R-g n ilc y c e Rla itn e to p
A1 A2 A3 A4 A5 B1 B2 B3 B4 B5 B6 B7 C1 C2 C3 C4 D
X X X X X MND MND MNR MNR MNR MND MND MND X X X X
RESULTS OF THE LCA - ENVIRONMENTAL IMPACT according to EN 15804+A2: 1 m³ flexen®PE
Parameter Unit A1-A3 A4 A5 C2 C3 C4 D
GWP-total kg CO 2 eq 6.51E+01 1.59E+00 0 1.47E-01 1.9E+00 0 -4.39E+01
GWP-fossil kg CO 2 eq 6.52E+01 1.59E+00 0 1.48E-01 1.88E+00 0 -4.35E+01
GWP-biogenic kg CO 2 eq -1.93E-01 -2.01E-02 0 -1.45E-03 2.62E-02 0 -3.71E-01
GWP-luluc kg CO 2 eq 7.38E-02 1.42E-02 0 9.97E-04 7.27E-04 0 -6.03E-03
ODP kg CFC11 eq 1.69E-08 2E-13 0 1.45E-14 7.76E-11 0 -2.66E-10
AP mol H+ eq 2.41E-01 1.87E-03 0 1.75E-04 2.69E-03 0 -6.04E-02
EP-freshwater kg P eq 2.64E-04 5.61E-06 0 5.29E-07 1.26E-05 0 -8.15E-05
EP-marine kg N eq 3.51E-02 6.36E-04 0 5.84E-05 1.07E-03 0 -1.77E-02
EP-terrestrial mol N eq 3.79E-01 7.51E-03 0 6.94E-04 1.09E-02 0 -1.84E-01
kg NMVOC
POCP 1.5E-01 1.91E-03 0 1.77E-04 2.6E-03 0 -5.77E-02
eq
ADPE kg Sb eq 1.81E-01 1.01E-07 0 1.49E-08 1.09E-06 0 -1.11E-05
ADPF MJ 2E+03 2.09E+01 0 1.94E+00 5.63E+01 0 -1.68E+03
m3 world eq
WDP 5.2E+00 1.85E-02 0 1.66E-03 1.36E-01 0 -7.42E-01
deprived
GWP = Global warming potential; ODP = Depletion potential of the stratospheric ozone layer; AP = Acidification potential of land and water; EP =
Eutrophication potential; POCP = Formation potential of tropospheric ozone photochemical oxidants; ADPE = Abiotic depletion potential for non-fossil
resources; ADPF = Abiotic depletion potential for fossil resources; WDP = Water (user) deprivation potential)
RESULTS OF THE LCA - INDICATORS TO DESCRIBE RESOURCE USE according to EN 15804+A2: 1 m³ flexen®PE
Parameter Unit A1-A3 A4 A5 C2 C3 C4 D
PERE MJ 2.73E+02 1.52E+00 0 1.35E-01 3.47E+01 0 -1.26E+02
PERM MJ 0 ND ND ND ND ND ND
PERT MJ 2.73E+02 1.52E+00 0 1.35E-01 3.47E+01 0 -1.26E+02
PENRE MJ 1.13E+03 2.1E+01 0 1.95E+00 5.63E+01 0 -1.68E+03
PENRM MJ 8.83E+02 ND ND ND ND ND ND
PENRT MJ 2.01E+03 2.1E+01 0 1.95E+00 5.63E+01 0 -1.68E+03
SM kg 9.01E+00 ND ND ND ND ND ND
RSF MJ 0 ND ND ND ND ND ND
6 Environmental Product Declaration - Adolf Würth GmbH & Co. KG - flexen®PE
NRSF MJ 0 ND ND ND ND ND ND
FW m3 3.47E-01 1.67E-03 0 1.56E-04 1.59E-02 0 -1.98E-01
PERE = Use of renewable primary energy excluding renewable primary energy resources used as raw materials; PERM = Use of renewable primary
energy resources used as raw materials; PERT = Total use of renewable primary energy resources; PENRE = Use of non-renewable primary energy
excluding non-renewable primary energy resources used as raw materials; PENRM = Use of non-renewable primary energy resources used as raw
materials; PENRT = Total use of non-renewable primary energy resources; SM = Use of secondary material; RSF = Use of renewable secondary fuels;
NRSF = Use of non-renewable secondary fuels; FW = Use of net fresh water
RESULTS OF THE LCA – WASTE CATEGORIES AND OUTPUT FLOWS according to EN 15804+A2:
1 m³ flexen®PE
Parameter Unit A1-A3 A4 A5 C2 C3 C4 D
HWD kg 1.8E-04 6.5E-11 0 1.03E-11 5.96E-09 0 -1.57E-07
NHWD kg 2.69E+00 3.2E-03 0 3.18E-04 7.46E-02 0 -4.63E-01
RWD kg 7.23E-02 3.93E-05 0 3.62E-06 1.31E-02 0 -1.4E-02
CRU kg ND ND ND ND ND ND ND
MFR kg ND ND 9.01E+00 ND 2.43E+01 ND ND
MER kg ND ND ND ND ND ND ND
EEE MJ ND ND ND ND ND ND ND
EET MJ ND ND ND ND ND ND ND
HWD = Hazardous waste disposed; NHWD = Non-hazardous waste disposed; RWD = Radioactive waste disposed; CRU = Components for re-use;
MFR = Materials for recycling; MER = Materials for energy recovery; EEE = Exported electrical energy; EET = Exported thermal energy
RESULTS OF THE LCA – additional impact categories according to EN 15804+A2-optional:
1 m³ flexen®PE
Parameter Unit A1-A3 A4 A5 C2 C3 C4 D
Disease
PM 1.12E-05 1.41E-08 0 1.34E-09 2.14E-08 0 -4.54E-07
incidence
IR kBq U235 eq 6.37E+00 5.86E-03 0 5.47E-04 9.12E-01 0 -1.39E+00
ETP-fw CTUe 1.18E+03 1.49E+01 0 1.38E+00 2.19E+01 0 -7.98E+02
HTP-c CTUh 3E-08 3.04E-10 0 2.84E-11 5.4E-10 0 -1.96E-08
HTP-nc CTUh 2.41E-06 1.63E-08 0 1.56E-09 1.67E-08 0 -9.14E-07
SQP SQP 1.76E+02 8.74E+00 0 8.22E-01 3.54E+01 0 -8.56E+01
PM = Potential incidence of disease due to PM emissions; IR = Potential Human exposure efficiency relative to U235; ETP-fw = Potential comparative
Toxic Unit for ecosystems; HTP-c = Potential comparative Toxic Unit for humans (cancerogenic); HTP-nc = Potential comparative Toxic Unit for humans
(not cancerogenic); SQP = Potential soil quality index
Disclaimer 1 – for the indicator “Potential Human exposure efficiency relative to U235”.This impact category deals mainly with the
eventual impact of low dose ionizing radiation on human health of the nuclear fuel cycle. It does not consider effects due to possible
nuclear accidents, occupational exposure or radioactive waste disposal in underground facilities. Potential ionizing radiation from the
soil, radon and from some construction materials is also not measured by this indicator.
Disclaimer 2 – for the indicators “abiotic depletion potential for non-fossil resources”, “abiotic depletion potential for fossil resources”,
“water (user) deprivation potential, deprivation-weighted water consumption”, “potential comparative toxic unit for ecosystems”,
“potential comparative toxic unit for humans – cancerogenic”, “Potential comparative toxic unit for humans - not cancerogenic”,
“potential soil quality index”. The results of this environmental impact indicator shall be used with care as theuncertainties on these
results are high as there is limited experience with the indicator. This EPD was created using a software tool.
6. LCA: Interpretation
The use of internal recycled material in flexen® PE reduces the module A1 to A3 shows that the production of raw materials
need for raw materials and avoids wasting resources. flexen® and their transport account for almost 96% of the impact Global
PE has a very low density, which means that little raw material Warming Potential. As the flexen® PE is fully recyclable;
is needed for high insulation efficiency, which results in the choice for the end of life was that of 100% recycling. This
significant energy savings. In addition, flexen® PE is largely avoids the use of new raw materials and or the exploitation of
made of low-density polyethylene, so it is fully recyclable and renewable or non-renewable resources. The end of life in 100%
can be recycled when it reaches the end of its life. As there is a landfill has a slight impact, especially from the point of view of
variation in density between the different references of the climate change. However, the 100% incineration scenario
flexen® PE range, a sensitivity analysis has been performed. has the greatest impact because during incineration there is a
The results of the LCA are given for 1m3 of product calculated significant release of carbon dioxide. The insulation with
with an average weighted foam density of 24,3 kg/m³. For the flexen® PE of the sanitary and heating piping contributes to a
lowest density, the impacts are lowered by 9,6 % and for the significant reduction of CO 2 emissions from the heating or
highest density the impacts should be majored by 27,3 %. Most cooling equipment, this is not considered in this LCA. It should,
references are very close to the average density, but all impact however, be taken into account in the calculation of
factors can be recalculated based on their density. When we environmental impacts of the complete heating and cooling
analyse the complete life cycle, we see that the most impacting systems or of the
part for all environmental impact factors is the production complete building. One way to continue to reduce the
module and more particularly the raw materials part. Regarding environmental impact of the flexen® PE would be to continue to
global warming for the complete life cycle, more than 95% diversify our energy sources by switching
comes from the production module 1,4% form transport to the more and more to renewable energies. To this end, after having
places of installation and 3,0% comes from the end of life. A greatly increased the number of photovoltaic panels, The
more in-depth analysis of the production production plant will acquire a cogeneration system. Looking for
7 Environmental Product Declaration - Adolf Würth GmbH & Co. KG - flexen®PE
more eco-responsible suppliers must also be put in place, as which is currently being carried out, should identify areas for
well as finding raw materials manufactured locally to avoid long- improvement and find solutions to achieve the goal of zero
distance transport carbon.
as much as possible. An analysis of the plant's carbon footprint,
7. Requisite evidence
7.1. VOC emissions after 28 days. Certificates are available on request. 7.1 VOC
Eurofins Product Testing A/S has tested a wide range and emissions
variety of typical PEF (Polyethylene foam) products marketed in For products used in indoor applications.
the EU from CEFEP (European Test procedure to AgBB diagram indicating the measuring
Group of PEF/FEF manufacturers) Based on the loading factor agency, date and results as a range of values. At least the
0.05m²/m3 following must be declared:
(determined after consideration of the real-life applications of 7.2 Leaching
PEF products (in living rooms) and recommendations by the According to EN13468 the content of water-soluble chloride
experts of the test institute) all results were found to be clearly ions for flexen® PE is <10mg/kg
below the limit values. For all samples below 100mg/m3 TVOC
8. References
EN 1602 building equipment and industrial installations.
EN 1602: 2013: Thermal insulating products for Determination of maximum service temperature for
building applications - Determination of the apparent preformed pipe insulation
density
EN 15804
EN ISO 8497 EN 15804: 2012-04 + A1 2014: Sustainability of
EN ISO 8497: Thermal insulation - Determination of construction works — Environmental Product
steady-state thermal transmission properties of thermal Declarations — Core rules for the product category of
insulation for circular pipes construction products
ISO 9001 CEN/TR 15941
ISO 9001: 2015: Quality management systems. CEN/TR 15941: Sustainability of construction works -
Environmental product declarations - Methodology for
EN 13472 selection and use of generic data
EN 13472 : Thermal insulating products for building equipment
and industrial installations - Determination of short term water CEN TS 16516
absorption by partial immersion of preformed pipe insulation CEN TS 16516: AgBB, ISO 16000-3, /ISO 16000-6/,
/ISO16000-9/, /ISO 16000-11/ Construction products -
EN 13468 Assessment of release of dangerous substances.
EN 13468 : Thermal insulating products for building equipment Determination of emissions into indoor air
and industrial installations - Determination of trace quantities of
water-soluble chloride, fluoride, silicate, and sodium ions and EN 16783: 2017
pH EN 16783: 2017 Thermal insulation products - Product
category rules (PCR) for factory made and in-situ
formed products for preparing environmental product
EN 13501-1 declarations
EN 13501-1:2007+A1: 2013 Fire classification of
construction products and building elements - Candidate list substances of very high concern
Classification using test data from reaction to fire tests SVCH: date: 08.07.2021) exceeding 0.1 percentage by mass
ISO 14001 CEFEP
ISO 14001: 2015 Environmental management CEFEP: European group of PEF and FEF manufacturers
systems.
Eurostat
EN ISO 14025 European Statistics: Recovery rates for packaging
EN ISO 14025: 2011-10: Environmental labels and waste Paper and cardboard packaging for the
declarations — Type III environmental declarations — European Union 27 countries 2014
Principles and procedures http://ec.europa.eu/eurostat/home
ISO 14040 Eurofins
ISO 14040: Environmental management — Life cycle Eurofins: Eurofins Scientific is a group of international life
assessment — Principles and framework sciences companies which provide a unique range of analytical
testing services to clients across multiple industries,
ISO 14044 http://www.eurofins.com
ISO 14044: Environmental management — Life cycle
assessment — Requirements and guidelines Gabi ts
GaBi 10 GaBi Software-System and Database for Life
EN 14707 Cycle Engineering Copyright © 1992-2021 Sphera
EN 14707: 2012: Thermal insulating products for Solutions Gmbh Version: 10.5.0.78 DB Schema 8007
8 Environmental Product Declaration - Adolf Würth GmbH & Co. KG - flexen®PE
of Institute Construction and Environment e.V. (IBU)
Institut Bauen und Umwelt Part B: Requirements on the EPD for Insulating
Institut Bauen und Umwelt e.V., Berlin(pub.): General materials made of foam plastics
Instructions for the EPD Programme of Institut Bauen Version 1.6 (Template) Version 1.2 (PCR specific)
und Umwelt e.V., Version 2.0 2021.
REACH
Ordinance on Biocide Products: No. 528/2012 According the European Chemicals Regulation REACH
manufacturers, importers and downstream users must register
Product Category Rules for Building-Related their chemicals and are responsible for their safe use.
Products and Services
Institute Construction and Environment e.V. (IBU) Sphera
Part A: Calculation Rules for the Life Cycle Sphera Solutions Gmbh. GaBi 10 LCI documentation.
Assessment and Requirements on the Project Report GaBi Databases (sphera.com) Stuttgart.
Version 1.7 The literature referred to in the Environmental Product
Declaration must be listed in full.Standards already fully quoted
PCR Guidance-Texts for Building-Related Products in the EPD do not need to be listed here again.
and Services The current version of PCR Part A and PCR Part B of the PCR
From the range of Environmental Product Declarations document on which they are based must be referenced.
9 Environmental Product Declaration - Adolf Würth GmbH & Co. KG - flexen®PE
Publisher
Institut Bauen und Umwelt e.V. +49 (0)30 3087748- 0
Hegelplatz 1 info@ibu-epd.com
10117 Berlin www.ibu-epd.com
Germany
Programme holder
Institut Bauen und Umwelt e.V. +49 (0)30 3087748- 0
Hegelplatz 1 info@ibu-epd.com
10117 Berlin www.ibu-epd.com
Germany
Author of the Life Cycle Assessment
Owner of the Declaration
Adolf Würth GmbH & Co. KG +49 7940/15-0
Reinhold-Würth-Str. 12-17 info@wuerth.com
74653 Künzelsau www.wuerth.de
Germany
10 Environmental Product Declaration - Adolf Würth GmbH & Co. KG - flexen®PE
