ENVIRONMENTAL PRODUCT DECLARATION
as per ISO 14025 and EN 15804+A2
Owner of the Declaration dormakaba International Holding GmbH
Publisher Institut Bauen und Umwelt e.V. (IBU)
Programme holder Institut Bauen und Umwelt e.V. (IBU)
Declaration number EPD-DOR-20220356-CBA3-EN
Issue date 14/04/2023
Valid to 13/04/2028
KTV Atrium Flex
dormakaba
www.ibu-epd.com | https://epd-online.com
General Information
dormakaba KTV Atrium Flex
Programme holder Owner of the declaration
IBU – Institut Bauen und Umwelt e.V. dormakaba International Holding GmbH
Hegelplatz 1 DORMA Platz 1
10117 Berlin 58256 Ennepetal
Germany Germany
Declaration number Declared product / declared unit
EPD-DOR-20220356-CBA3-EN 1 piece of the product: KTV Atrium Flex All Glass Revolving Door, with four
(4) door leaves and a diameter of 3000 mm and a height of 2200 mm,
consisting of the following items:
• Drum wall
• Canopy construction
• Light ring
• Door wings
• Turnstile fittings
• KT FLEX Direct drive unit
• Electric accessories / sensors
• Floor ring
• Claddings
• Product packaging
This declaration is based on the product category rules: Scope:
Automatic doors, automatic gates, and revolving door systems, This Environmental Product Declaration refers to a specific KTV Atrium
01/08/2021 Flex All Glass Revolving Door manufactured by dormakaba. The
(PCR checked and approved by the SVR) production site is located in Sofia (Bulgaria).
Data represents the year 2022.
Issue date The owner of the declaration shall be liable for the underlying information
and evidence; the IBU shall not be liable with respect to manufacturer
14/04/2023
information, life cycle assessment data and evidences.
The EPD was created according to the specifications of EN 15804+A2. In
Valid to
the following, the standard will be simplified as EN 15804.
13/04/2028
Verification
The standard EN 15804 serves as the core PCR
Independent verification of the declaration and data according to ISO
14025:2011
internally X externally
Dipl.-Ing. Hans Peters
(Chairman of Institut Bauen und Umwelt e.V.)
Florian Pronold Dr.-Ing. Wolfram Trinius,
(Managing Director Institut Bauen und Umwelt e.V.) (Independent verifier)
1 Environmental Product Declaration - dormakaba - KTV Atrium Flex
Product
• Public buildings
Product description/Product definition • Hospitals
The KTV Atrium Flex door range is a breakthrough in design • Hotels
with technology: The revolving door is driven by an Automatic revolving doors are used to control the pedestrian
electromagnetic direct drive - the dormakaba FLEX Direct Drive flow in combination with an optimal thermal separation of the
technology complements the design intent of modern inside and outside climates during normal use.
architecture. It is unique, elegant and leaves an impression that
is lasting and timeless. Technical Data
Advanced German drive technology using innovative magnetic
For the use and application of the product the respective levitation technology, the door panels are directly driven by
national provisions at the place of use apply. For the KTV contactless magnetic fields, instead of conventional belt and
Atrium Flex the standards which can be applied are the gear system, realizing an extremely compact low-wear
following: automation system that delivers quiet motion millions of times
over.
• 20111765/EU ROHS3 Directive
• ISO 13849-1: Safety of machinery - Safety-related parts
of control systems - Part 1: General principles for
Base materials/Ancillary materials
design.
The major material composition including the packaging of the
• ISO 12100: Safety of machinery - Basic concepts - Risk
product is listed below.
assessment and risk reduction
• EN 16005: Power operated pedestrian doorsets - Safety Name Value Unit
in use - Requirements and test methods Glass 66 %
• EN 61000 - 6 - 2: Electromagnetic compatibility (EMC). Packaging 10 %
Part 6-2: Generic standards: Interference resistance for
Stainless steel 9 %
industrial environments
Aluminium 8 %
• EN 61000 - 6 - 3: Electromagnetic compatibility (EMC).
Part 6-3: Generic standards: Emission standard for Steel 3 %
residential, commercial and light-industrial Plastic 2 %
environments. Electronics 2 %
• EN 61000 - 3 - 2: Electromagnetic compatibility-3-2:
The KTV Atrium Flex includes partial articles which contain
Limits - Limits for harmonic current emissions
substances listed in the Candidate List of REACH Regulation
• EN 61000 - 3 - 3: Electromagnetic compatibility-3-3:
1907/2006/EC (date: 17.01.2023) exceeding 0.1 percentage by
Limits - Limitation of voltage changes, voltage
mass: yes
fluctuations and flicker in public low-voltage supply
systems • Lead (Pb): 7439921(CASNo.) is included in some of the
• EN 55022: Information technology equipment - Radio alloys used. The concentration of lead in each individual
disturbance characteristics - Limits and methods of alloy does not exceed 4 %(by mass).
measurement • Dodecamethylcyclotetrasiolxane:
• EN 60335 - 1: Safety of household and similar electrical 540-97-6 (CASNo.) is included in the glue, exceeding
appliances. Part 1: General requirements 0,1% (by mass).
• EN 60335-2-103: Household and similar electrical
• 2,2,4,4,6,6,8,8,10,10-decampethylcyclopentasiloxane:
appliances. Safety-Particular requirements for drives for
541-02-6 (CASNo.) is included in the glue, exceeding
gates, doors and windows
0,1% (by mass).
• DIN 18650-1: Powered pedestrian doors.
Part 1: Product requirements and test • Octamethylcyclotetrasiloxane:
methods 556-67-2 (CASNo.) is included in the glue, exceeding
• DIN 18650-2: Powered pedestrian doors. 0,1% (by mass).
Part 2: Safety at powered pedestrian doors The Candidate List can be found on the ECHA website
The CE-marking takes into account the proof of conformity with address: https://echa.europa.eu/de/home.
the respective harmonized norms based on the legal provisions
Reference service life
above.
The reference service life of the KTV Atrium Flex amounts to 20
years and depends on the application and frequency of use.
Application Regular maintenance is advised to ensure the life expectancy
of 20 years. For repairs and renewals, suitable spare parts are
The KTV Atrium Flex is ideal for modern entrances.
available. The product is tested and certified to EN 16005,
Typical applications include:
meaning they are designed to withstand a minimum of 10
• Office / commercial buildings million cycles.
• Airports
LCA: Calculation rules
Declared Unit
The declared unit is 1 piece of the product: KTV Atrium Flex
2 Environmental Product Declaration - dormakaba - KTV Atrium Flex
Name Value Unit — A5, installation into the building; including provision of all
Declared unit for revolving door system* 6.6 m2 materials, products and energy, as well as waste processing up
to the end-ofwaste state or disposal of final residues during the
Mass of the entire system 1615.72 kg
construction process stage.
Grammage of the components 244.8 kg/m2
Dimension for revolving door, diameter 3000 mm Use stage - Module B6
Dimensions for revolving door, height 2200 mm The use stage related to the operation of the buildingincludes:
— B6, operational energy use
Layer thickness 1 m
* Area represents the cross-sectional area of the door, which is End-of-life stage– Modules C1-C4 and D
designed to fit in an opening of 3000 mm wide by 2200 mm The end-of-life stage includes:
high. — C1, de-construction, demolition:
— C2, transport to waste processing;
— C3, waste processing for reuse, recovery and/orrecycling;
— C4, disposal; including provision and all transport, provision
System boundary
of all materials, products and related energy and water use.
The type of EPD is: cradle to gate with options, modules C1– Module D (Benefits and loads beyond the system boundary)
C4, and module D (A1–A3 + C + D andadditional modules: A4 includes:
+ A5 + B6) — D, recycling potentials, expressed as net
impactsand benefits.
Production - Module A1-A3
The product stage includes: Geographic Representativeness
— A1, raw material extraction, processing and mechanical Land or region, in which the declared product system is
treatments, processing of manufactured, used or handled at the end of the product´s
secondarymaterial input (e.g. recycling processes), lifespan: Global
— A2, transport to the manufacturer,
— A3, manufacturing and assemblyincluding provision of all
materials, products and energy, as well as waste processing up Comparability
to the end-of waste state. Basically, a comparison or an evaluation of EPD data is only
possible if all the data sets to be compared were created
Construction stage - Modules A4-A5 according to EN 15804 and the building context, respectively
The construction process stage includes: the product-specific characteristics of performance, are taken
— A4, transport to the building site; into account. Background database: GaBi, SP40.
LCA: Scenarios and additional technical information
Operational energy use (B6)
Characteristic product properties of biogenic carbon
Name Value Unit
Electricity consumption (per year) 177.05 kWh
Information on describing the Biogenic Carbon Content at
factory gate Days per year in use 365 days
Name ValueUnit On mode per day 2,5 h
Biogenic carbon content in accompanying kg Idle mode per day 10,5 h
68.08
packaging C Off mode per day 11 h
On mode power 31,49 W
Idle mode power 18,9 W
Off mode power 18,9 W
Transport to the building site (A4)
Additional technical information for the declared modules.
Name Value Unit
Litres of fuel (per 1 kg) 0.00276 l/100km End of life (C1-C4)
Transport distance 100 km C1: The product expansion depends on the building. The
product share is so low that no environmental burden is
Capacity utilisation (including empty runs) 55 %
assumed.
The product is transported via truck from the production site in
Name Value Unit
Bulgaria to the European sales markets. In order to allow
Collected separately waste type waste type 1451.5 kg
scaling to a specific point of installation 100 km are declared.
Recycling 333 kg
Energy recovery 38.5 kg
Installation into the building (A5)
Landfilling 1080 kg
Name Value Unit
Transport to waste management 50 km
Waste packaging (paper and plastic) 1,2 kg
Wooden pallets 160 kg The product is disassembled in a recycling process. Material
recycling is then assumed for the metals and electronics. The
plastic components are assumed to be incinerated with energy
Reference service life recovery. Glass and electromechanics are landfilled.
Name Value Unit Region for the End of Life is: Global.
Life Span according to the manufacturer 20 a
3 Environmental Product Declaration - dormakaba - KTV Atrium Flex
Collection rate is 100%.
Reuse, recovery and/or recycling potentials (D), relevant
scenario information
Name Value Unit
Recycling 100 %
4 Environmental Product Declaration - dormakaba - KTV Atrium Flex
LCA: Results
DESCRIPTION OF THE SYSTEM BOUNDARY (X = INCLUDED IN LCA; MND = MODULE OR INDICATOR NOT DECLARED; MNR
= MODULE NOT RELEVANT)
Benefits and
Construction loads beyond
Product stage Use stage End of life stage
process stage the system
boundaries
la ire ta m w a Ry lp p u s tro p s n a rT g n iru tc a fu n a M e h t m o rf tro p s n a rTe tis e h t o t e ta g y lb m e s s A e s U e c n a n e tn ia M ria p e R tn e m e c a lp e R tn e m h s ib ru fe R y g re n e la n o ita re p Oe s u re ta w la n o ita re p Oe s u n o itc u rts n o c -e Dn o itilo m e d tro p s n a rT g n is s e c o rp e ts a W la s o p s iD -e s u e R-y re v o c e R-g n ilc y c e Rla itn e to p
A1 A2 A3 A4 A5 B1 B2 B3 B4 B5 B6 B7 C1 C2 C3 C4 D
X X X X X MND MND MNR MNR MNR X MND X X X X X
RESULTS OF THE LCA - ENVIRONMENTAL IMPACT according to EN 15804+A2: 1 piece KTV Atrium Flex
Parameter Unit A1-A3 A4 A5 B6 C1 C2 C3 C4 D
GWP-total kg CO 2 eq 4.76E+03 1.41E+01 2.62E+02 1.43E+03 0 6.35E+00 9.8E+01 1.65E+01 -1.68E+03
GWP-fossil kg CO 2 eq 4.96E+03 1.35E+01 4.86E+00 1.43E+03 0 6.07E+00 9.8E+01 1.64E+01 -1.67E+03
GWP-biogenic kg CO 2 eq -2.03E+02 6.24E-01 2.57E+02 4.75E+00 0 2.81E-01 2E-03 5.6E-02 2.99E-01
GWP-luluc kg CO 2 eq 3.46E+00 3.22E-04 3E-03 2.07E+00 0 1.45E-04 6E-03 4.7E-02 -1.52E+00
ODP kg CFC11 eq 2.63E-09 1.43E-15 3.83E-14 3.14E-11 0 6.41E-16 4.94E-14 6.09E-14 -6.92E-09
AP mol H+ eq 2.87E+01 1.4E-02 4.4E-02 3.15E+00 0 6E-03 1.7E-02 1.18E-01 -6.63E+00
EP-freshwater kg P eq 4.31E-03 2.89E-06 6.72E-06 4E-03 0 1.3E-06 7.88E-06 2.82E-05 -1E-03
EP-marine kg N eq 5.66E+00 4E-03 1.3E-02 6.99E-01 0 2E-03 4E-03 3E-02 -9.49E-01
EP-terrestrial mol N eq 6.35E+01 4.8E-02 1.81E-01 7.34E+00 0 2.2E-02 7.9E-02 3.33E-01 -1.03E+01
kg NMVOC
POCP 1.42E+01 1.2E-02 3.5E-02 1.92E+00 0 5E-03 1.1E-02 9.2E-02 -2.92E+00
eq
ADPE kg Sb eq 7.7E-02 4.05E-07 6.06E-07 4.13E-04 0 1.82E-07 6.78E-07 1.48E-06 -3.1E-02
ADPF MJ 6.5E+04 1.92E+02 6.62E+01 2.51E+04 0 8.61E+01 4.54E+01 2.15E+02 -2.26E+04
m3 world eq
WDP 1.09E+03 2.6E-02 2.88E+01 3.11E+02 0 1.2E-02 1E+01 1.72E+00 -3.28E+02
deprived
GWP = Global warming potential; ODP = Depletion potential of the stratospheric ozone layer; AP = Acidification potential of land and water; EP =
Eutrophication potential; POCP = Formation potential of tropospheric ozone photochemical oxidants; ADPE = Abiotic depletion potential for non-fossil
resources; ADPF = Abiotic depletion potential for fossil resources; WDP = Water (user) deprivation potential)
RESULTS OF THE LCA - INDICATORS TO DESCRIBE RESOURCE USE according to EN 15804+A2: 1 piece KTV Atrium Flex
Parameter Unit A1-A3 A4 A5 B6 C1 C2 C3 C4 D
PERE MJ 1.37E+04 6.04E-01 2.11E+03 1.11E+04 0 2.72E-01 1.18E+01 2.82E+01 -7.96E+03
PERM MJ 2.09E+03 0 -2.09E+03 0 0 0 0 0 0
PERT MJ 1.58E+04 6.04E-01 1.24E+01 1.11E+04 0 2.72E-01 1.18E+01 2.82E+01 -7.96E+03
PENRE MJ 6.37E+04 1.92E+02 6.63E+01 2.51E+04 0 8.62E+01 1.37E+03 2.16E+02 -2.26E+04
PENRM MJ 1.32E+03 0 0 0 0 0 -1.32E+03 0 0
PENRT MJ 6.51E+04 1.92E+02 6.63E+01 2.51E+04 0 8.62E+01 4.54E+01 2.16E+02 -2.26E+04
SM kg 7.61E+01 0 0 0 0 0 0 0 0
RSF MJ 0 0 0 0 0 0 0 0 0
NRSF MJ 0 0 0 0 0 0 0 0 0
FW m3 4.57E+01 1E-03 6.78E-01 1.28E+01 0 4.87E-04 2.4E-01 5.4E-02 -2.14E+01
PERE = Use of renewable primary energy excluding renewable primary energy resources used as raw materials; PERM = Use of renewable primary
energy resources used as raw materials; PERT = Total use of renewable primary energy resources; PENRE = Use of non-renewable primary energy
excluding non-renewable primary energy resources used as raw materials; PENRM = Use of non-renewable primary energy resources used as raw
materials; PENRT = Total use of non-renewable primary energy resources; SM = Use of secondary material; RSF = Use of renewable secondary fuels;
NRSF = Use of non-renewable secondary fuels; FW = Use of net fresh water
RESULTS OF THE LCA – WASTE CATEGORIES AND OUTPUT FLOWS according to EN 15804+A2:
1 piece KTV Atrium Flex
Parameter Unit A1-A3 A4 A5 B6 C1 C2 C3 C4 D
HWD kg 1.46E-04 1.86E-08 8.01E-08 1.04E-05 0 8.36E-09 1.73E-07 3.29E-06 -7.37E-05
NHWD kg 7.03E+02 2E-02 5.16E+00 1.78E+01 0 9E-03 1.02E+01 1.08E+03 -2.94E+02
RWD kg 1.81E+00 2.06E-04 4E-03 3.8E+00 0 9.25E-05 2E-03 2E-03 -1.57E+00
CRU kg 0 0 0 0 0 0 0 0 0
MFR kg 0 0 0 0 0 0 3.32E+02 0 0
MER kg 0 0 0 0 0 0 0 0 0
EEE MJ 0 0 3.65E+02 0 0 0 1.82E+02 0 0
EET MJ 0 0 6.57E+02 0 0 0 4.17E+02 0 0
5 Environmental Product Declaration - dormakaba - KTV Atrium Flex
HWD = Hazardous waste disposed; NHWD = Non-hazardous waste disposed; RWD = Radioactive waste disposed; CRU = Components for re-use;
MFR = Materials for recycling; MER = Materials for energy recovery; EEE = Exported electrical energy; EET = Exported thermal energy
RESULTS OF THE LCA – additional impact categories according to EN 15804+A2-optional:
1 piece KTV Atrium Flex
Parameter Unit A1-A3 A4 A5 B6 C1 C2 C3 C4 D
Disease
PM 2.81E-04 7.11E-08 2.99E-07 2.64E-05 0 3.2E-08 2.23E-07 1.46E-06 -1.16E-04
incidence
IR kBq U235 eq 3.09E+02 2.9E-02 5.78E-01 6.24E+02 0 1.3E-02 1.52E-01 2.52E-01 -3.1E+02
ETP-fw CTUe 5.4E+04 1.36E+02 3.14E+01 1.07E+04 0 6.1E+01 1.7E+01 1.23E+02 -9.37E+03
HTP-c CTUh 2.11E-04 2.55E-09 2.4E-09 2.96E-07 0 1.15E-09 1.48E-09 1.82E-08 -1.6E-06
HTP-nc CTUh 1.35E-04 1.09E-07 1.5E-07 1.09E-05 0 4.91E-08 1.49E-07 2.01E-06 -1.14E-05
SQP SQP 3.86E+04 4.92E-01 1.84E+01 7.98E+03 0 2.21E-01 1.36E+01 4.49E+01 -1.92E+03
PM = Potential incidence of disease due to PM emissions; IR = Potential Human exposure efficiency relative to U235; ETP-fw = Potential comparative
Toxic Unit for ecosystems; HTP-c = Potential comparative Toxic Unit for humans (cancerogenic); HTP-nc = Potential comparative Toxic Unit for humans
(not cancerogenic); SQP = Potential soil quality index
Disclaimer 1 – for the indicator “Potential Human exposure efficiency relative to U235”. This impact category deals mainly with the
eventual impact of low-dose ionizing radiation on human health of the nuclear fuel cycle. It does not consider effects due to possible
nuclear accidents, occupational exposure or radioactive waste disposal in underground facilities. Potential ionizing radiation from the
soil, radon and from some construction materials is also not measured by this indicator.
Disclaimer 2 – for the indicators “abiotic depletion potential for non-fossil resources”, “abiotic depletion potential for fossil resources”,
“water (user) deprivation potential, deprivation-weighted water consumption”, “potential comparative toxic unit for ecosystems”,
“potential comparative toxic unit for humans – cancerogenic”, “Potential comparative toxic unit for humans - not cancerogenic”,
“potential soil quality index”. The results of this environmental impact indicator shall be used with care as the uncertainties on these
results are high as there is limited experience with the indicator.
This EPD was created using a software tool.
References
ISO 14025
DIN EN ISO 14025:2011-10, Environmental labels and EN 61000-3-3
declarations — Type III environmental declarations — EN 61000-3-3: Electromagnetic compatibility-3-3: Limits -
Principles and procedures Limitation of voltage changes, voltage fluctuations and flicker in
public low-voltage supply systems.
EN 15804
EN 15804+A2:2019+AC:2021, Sustainability of construction EN 61000-6-2
works — Environmental Product Declarations — Core rules for EN 61000-6-2: Electromagnetic compatibility (EMC). Part 6-2:
the product category of construction products Generic standards: Interference resistance for industrial
environments.
DIN 18650-1
DIN 18650-1/: Powered pedestrian doors. Part 1: Product EN 61000-6-3
requirements and test methods. EN 61000-6-3: Electromagnetic compatibility (EMC). Part 6-3:
Generic standards: Emission standard for residential,
DIN 18650-2 commercial and light-industrial environments.
DIN 18650-2/: Powered pedestrian doors. Part 2: Safety at
powered pedestrian doors ISO 9001
ISO 9001: Quality management systems.
EN 16005
EN 16005: Power operated pedestrian doorsets - Safety in ISO 12100
use - Requirements and test methods. ISO 12100: Safety of machinery - Basic concepts - Risk
assessment and risk reduction.
EN 55022
EN 55022: Information technology equipment - Radio ISO 13849-1
disturbance characteristics - Limits and methods of ISO 13849-1: Safety of machinery - Safety-related parts of
measurement. control systems - Part 1: General principles for design.
EN 60335 IEC 60335-2-103
EN 60335 - 1: Safety of household and similar electrical IEC 60335-2-103: Household and similar electrical appliances.
appliances. Part 1: General requirements. Safety. Part 2-103: Particular requirements for drives for gates,
doors and windows.
EN 60335-2-103
EN 60335-2-103: Household and similar electrical appliances. REACH Regulation
Safety. Particular requirements for drives for gates, doors and REACH Regulation (EC) No 1907/2006 of the European
windows. Parliament and of the Council on the Registration, Evaluation,
Authorisation and Restriction of Chemicals.
EN 61000-3-2
EN 61000-3-2: Electromagnetic compatibility-3-2: Limits - Limits RoHS 2011/65/EU
for harmonic current emissions. RoHS 2011/65/EU, Directive on the restriction of the use of
6 Environmental Product Declaration - dormakaba - KTV Atrium Flex
certain hazardous substances in electrical and electronic GaBi life cycle inventory data documentation
equipment. (https://www.gabisoftware.
com/support/gabi/gabidatabase- 2020-lci-documentation/).
European Chemicals Agency (ECHA)
https:echa.europa.eu/de/home LCA-tool dormakaba
LCA tool, ENS (doors) Tool No.: IBU-DOR-202107-LT1-EN
Further References Developed by Sphera Solutions GmbH.
IBU 2021 PCR Part A
General Instructions for the EPD programme of Institut Bauen PCR – Part A: Calculation Rules for the Life Cycle Assessment
und Umwelt e.V. and Requirements on the Project Re-port according to EN
Version 2.0, Berlin: Institut Bauen und Umwelt e.V., 2021. 15804+A2:2019, Version 1.0, Institut Bauen und Umwelt e.V.,
www.ibu-epd.com www.ibu-epd.com.
GaBi PCR Part B
Sphera Solutions GmbH Gabi Software System and Database PCR – Part B: Requirements on the EPD for Automatic doors,
for Life Cycle Engineering 1992-2020 Version 10.0.0.71 automatic gates, and revolving door systems, 08/2021, Institut
University of Stuttgart Leinfelden-Echterdingen Bauen und Umwelt e.V., www.ibu-epd.com.
GaBi ts documentation
7 Environmental Product Declaration - dormakaba - KTV Atrium Flex
Publisher
Institut Bauen und Umwelt e.V. +49 (0)30 3087748- 0
Hegelplatz 1 info@ibu-epd.com
10117 Berlin www.ibu-epd.com
Germany
Programme holder
Institut Bauen und Umwelt e.V. +49 (0)30 3087748- 0
Hegelplatz 1 info@ibu-epd.com
10117 Berlin www.ibu-epd.com
Germany
Author of the Life Cycle Assessment
dormakaba International Holding GmbH +49 2333 793-0
DORMA Platz 1 info.de@dormakaba.com
58256 Ennepetal www.dormakaba.com
Germany
Owner of the Declaration
dormakaba International Holding GmbH +49 2333 793-0
DORMA Platz 1 info.de@dormakaba.com
58256 Ennepetal www.dormakaba.com
Germany
8 Environmental Product Declaration - dormakaba - KTV Atrium Flex
