ENVIRONMENTAL PRODUCT DECLARATION
as per ISO 14025 and EN 15804+A2
Owner of the Declaration IGI - The Global Wallcoverings Association
Publisher Institut Bauen und Umwelt e.V. (IBU)
Programme holder Institut Bauen und Umwelt e.V. (IBU)
Declaration number EPD-IGI-20230434-IBG1-EN
Issue date 18/01/2024
Valid to 17/01/2029
Vinyl wallcoverings on non-woven backing
IGI - The Global Wallcoverings Association
www.ibu-epd.com | https://epd-online.com
1. General Information
IGI - The Global Wallcoverings Association Vinyl wallcoverings on non-woven backing
Programme holder Owner of the declaration
IBU – Institut Bauen und Umwelt e.V. IGI - The Global Wallcoverings Association
Hegelplatz 1 Chaussée de Louvain 426
10117 Berlin 1380 LASNE
Germany Belgium
Declaration number Declared product / declared unit
EPD-IGI-20230434-IBG1-EN The declared unit is 1m² (square meter) decorative vinyl based
wallcovering on non-woven backing including packaging.
This declaration is based on the product category rules: Scope:
Wall coverings, 01/08/2021 This EPD focuses on the production, transport and disposal of a weighted
(PCR checked and approved by the SVR) average of 1m² vinyl wallcoverings on non-woven backing of participating
members of the IGI - The Global Wallcoverings Association.
16 out of 71 IGI-members are involved in this EPD: A.S. Création Tapeten
Issue date AG (DE), Anstey Wallpaper Co. Ltd. (GB), BN International (NL), Decoprint
NV (BE), Erismann & Cie. GmbH (DE), Graham & Brown Ltd. (GB),
18/01/2024
Grandeco NV (BE), JV S.p.A. (IT), Marburger Tapetenfabrik J.B. Schaefer
GmbH & Co. KG (DE), Muraspec Decorative Solutions Ltd. (GB), Rasch
GmbH & Co. KG (DE), Roysons Corporation (US), UGÉPA SA (FR), Versa
Valid to
Wallcovering (US), York Wallcoverings (US), Zambaiti Parati S.p.A. (IT).
17/01/2029 The technical properties are displayed in chapter 2.3.
The owner of the declaration shall be liable for the underlying information
and evidence; the IBU shall not be liable with respect to manufacturer
information, life cycle assessment data and evidences.
The EPD was created according to the specifications of EN 15804+A2. In
the following, the standard will be simplified as EN 15804.
Verification
The standard EN 15804 serves as the core PCR
Independent verification of the declaration and data according to ISO
14025:2011
Dipl.-Ing. Hans Peters
(Chairman of Institut Bauen und Umwelt e.V.) internally X externally
Florian Pronold Prof. Dr. Birgit Grahl,
(Managing Director Institut Bauen und Umwelt e.V.) (Independent verifier)
1 Environmental Product Declaration - IGI - The Global Wallcoverings Association - Vinyl wallcoverings on non-woven backing
2. Product
or:
2.1 Product description/Product definition
Vinyl wallcoverings on non-woven backing according to EN 1b
15102 involve plasticized PVC (vinyl) and a non-woven base. A Performance Category I, II, III, IV, V or VI as described in Table
non-woven base is a substrate composed of a blend of 1 of F 793-0-06 have to be declared.
cellulose and polyester fibres. Non-woven wallcovering is
available with relief or flat vinyl designs. The vinyl on non- 2.4 Delivery status
woven wallcovering is dimensionally stable to aqueous paste The products declared are provided within the following
and does not require a soak time. When the wallcovering is to dimensions:
be changed it can be stripped in its entirety by peeling the
wallcovering lengths from the wall. This property as defined in
EN 235 is strippable.
For the placing on the market of the product in the European
Union/European Free Trade Association (EU/EFTA) (with the
exception of Switzerland) Regulation (EU) No. 305/2011 (CPR) This table contains the range of all wallcoverings examined. For
applies. The product needs a Declaration of Performance more precise information please contact the specific
taking into consideration EN 15102 and CE-marking. manufacturer.
For the application and use the respective national provisions
2.5 Base materials/Ancillary materials
apply.
For the placing on the market in Great Britain the product The weighted average of the primary product components is
needs a Declaration of Performance taking into consideration shown in the following table, in percentage:
BS EN 15102 and UK Conformity Assessed (UKCA) marking. Name ValueUnit
For placing on the market in Northern Ireland the product needs
Carrier material (Non-Woven, 80% Paper 20%
a Declaration of Performance taking into consideration (BS) EN 25 %
PET)
15102 and CE or CE and UK Northern Ireland (UKNI) marking.
Packaging 6 %
For the placing on the market in the USA the product has to
Additives 32 %
conform to ASTM F 1141 – 93 Standard Specification for
Wallcovering and ASTM F 793 – 06 Standard Classification of PVC plastisol 33 %
Wall Covering by Use Characteristics. Ink & Pigment 3 %
Sum 100 %
2.2 Application
Wallcoverings are used for the decorative wall design of interior Pallets were considered as part of the packaging.
spaces in private or commercial use.
This product contains substances listed in the candidate list
2.3 Technical Data (date: 06.12.2023) exceeding 0.1 percentage by mass: no.
Name Value Unit This product contains other CMR substances in categories 1A
or 1B that are not on the candidate list, exceeding 0.1
Measures by categories EN 233 category 1 - 3 -
percentage by mass: no.
Straightness and parallelism in mm. equal or less than
- Biocide products were added to this construction product or it
according to EN 12956/ 1
has been treated with biocide products (this then concerns a
Washability according to EN 12956 Spongeable to - treated product as defined by the (EU) Ordinance on Biocide
extra-scrubbable Products No. 528/2012): no.
Colour fastness to light according to Ancillary materials of the phthalate chemical group, specifically
3 - 6 -
EN ISO 105-B02 Diisononyl phthalate (DINP) and Dioctyl Terephthalate (DOTP),
Migration of heavy metals and certain remain on the product and serve the function of softeners.
fulfills the norm -
other elements to EN 12149 Plasticizers can also be found in the products, in the plastisol
used for vinyl finishing.
Vinyl chloride monomer (VCM)
This EPD is a weighted average of a Manufacturer Group
content max. < 0,2 mg/m² according fulfills the norm -
regarding several producers and product references. Therefore,
to EN 12149
it cannot be ruled out that individual wallcoverings may contain
Emissions of formaldehyde max.
fulfills the norm - small amounts (>0.1% of product weight) of substances that
< 120 mg/kg according to EN 12149
are included in the Substance of Very High Concern SVHC
In case of multiple answers, values need to be examined candidate list, the CMR substances in categories 1A or 1B list
depending on the manufacturer. or ancillary materials and additives serving the function of fire
retardants, softeners or biocides.
Products manufactured for the USA need to be in accordance This can be attributed, for example, to the contents of used
with ASTM F 793-0-06 Table 1 Classification Criteria. waste paper. Further information can be obtained from the
respective manufacturer.
Depending on whether products are intended for the European,
UK or US markets, the following performance data must be 2.6 Manufacture
declared. The manufacturing process can be described with the help of
the following graphic:
1a:Product according to the CPR, based on (BS) EN 15102:
Performance data of the product in accordance with the
Declaration of Performance with respect to its Essential
Characteristics according to EN 15102
2 Environmental Product Declaration - IGI - The Global Wallcoverings Association - Vinyl wallcoverings on non-woven backing
Description of the influences on the ageing of the product when
applied in accordance with the rules of technology.
2.13 Extraordinary effects
Fire
The reaction to fire performance according to EN 13501 is
shown in the following table:
Fire protection
Name Value
Building material class B-D
Burning droplets s1-s3
Smoke gas development d0-d2
This table contains the range of all wallcoverings examined. For
more precise information please contact the specific
The order of manufacture may change and can slightly deviate
manufacturer.
for different producers.
2.7 Environment and health during manufacturing For USA information on fire performanceaccording to ASTM E
84 Test method for Surface Burning Characteristics of Building
Compliance with statutory health and safety for personnel is
Materials.
ensured. Further, the energy and environmental management
is certified for some members according to ISO 14001 and ISO
50001.
Water
For greater detail please contact the specific manufacturer.
The product is not water resistant. There is no risk of a
2.8 Product processing/Installation hazardous environmental impact in the event of water flooding.
Depending on the manufacturers suggestion, the adhesive is
applied to the back of the wallcovering or the substrate using a Mechanical destruction
wallpaper brush or short-napped roller. The wallcovering is There is no risk of a hazardous environmental impact following
pressed against the wall and is cut along the top and bottom unforeseen mechanical destruction.
edges to fit the wall.
2.14 Re-use phase
2.9 Packaging The product is not re-usable.
Product is wrapped in shrink wrap film, packed in corrugated
2.15 Disposal
cardboard boxes and palletised.
Wallcoverings are subject to the waste code 170904 (mixed
2.10 Condition of use construction and demolition waste other than those mentioned
There are no special features to be noted within the limits of in 170901, 170902 and 170903) in accordance with the
normal and customary usage. European Waste Catalogue (EWC).
2.11 Environment and health during use Wallcoverings can therefore be disposed of as normal
No environmental problems can be expected when the product household waste, that is in the dustbin or in additional refuse
is handled and used sacks. Used wallcoverings should not be placed in the waste
properly. paper bank. Most household waste is incinerated or landfilled
depending on regional legal regulations in the EU or in the US.
2.12 Reference service life
Given the wallcovering is professionally installed, the reference 2.16 Further information
service life is 10 years according to the German Sustainable For further information please visit www.igiwallcoverings.org.
Building Assessment System (BNB).
3. LCA: Calculation rules
datasets correspond to all regarded regions.
3.1 Declared Unit
The declared unit is 1 m² of wallcovering including packaging. 3.2 System boundary
The model is based on a weighted average of the produced Type of the EPD: cradle to gate - with Options.
square meters of each participating manufacturer. The EPD is considered a declaration of an average product as
calculated from the output of several manufacturers (2b).
Declared unit
Name Value Unit
Modules A1-3, A4 and A5
Declared unit 1 m2 The product stage begins with the consideration of the
Grammage 0.223 kg/m2 production of the necessary raw materials and energies
including all corresponding upstream processes as well as
Conversion factor to 1 kg 4.484 -
transport.
Layer thickness 0.001 m
Furthermore, the entire production phase was investigated,
Density 2231 kg/m3 including the treatment of production waste until reaching the
end-of-waste status (EoW). In addition, distribution transport
The production processes and location may vary between
and installation in the building were taken into account.
individual companies. The weighted average represents the
most likely scenario by production volumes and the selected
Modules C1-C4
3 Environmental Product Declaration - IGI - The Global Wallcoverings Association - Vinyl wallcoverings on non-woven backing
The modules include the environmental impacts of the reoval Data collection for the investigated products was carried out on
and waste treatment until reaching the end-of-waste status the basis of evaluations of the internal production and
(EoW) including the associated transport at the end of the environmental data, the collection of LCA-relevant data within
product life cycle. the supply chain as well as through the measurement of
relevant energy supply data. The collected data were checked
Module D for plausibility and consistency. A good representation is to be
Calculation of potential benefits through the generated energy assumed.
(electric & thermic) by the incineration processes in the life The data were collected in 2022 and refer to the calendar year
cycle stages in A5 C3 and C4. The burdens resulting from the 2021.
waste-to-energy plants are assigned in module C3 or C4 in
case of landfill gas combustion. 3.7 Period under review
The LCA data were collected for the calendar year 2021.
3.3 Estimates and assumptions
'Non-woven' lacks information on the proportions of cellulose 3.8 Geographic Representativeness
and polyester. According to one manufacturer it contains 80% Land or region, in which the declared product system is
cellulose and 20% polyester (PET). These proportions were manufactured, used or handled at the end of the product´s
applied to all other non-woven carrier materials. lifespan: Global
Most solvents were modelled as a generic mix of solvents.
3.4 Cut-off criteria 3.9 Allocation
No materials were cut-off from the study. No energy Potential benefits resulting from the thermal utilization of the
consumption was neglected. packaging waste (module A5) as well as from the thermal
utilization or landfilling of the wallcoverings at the end of life
3.5 Background data (modules C3 and C4) are allocated to module D.
For modelling the lifecycle, the LCA for Experts Software
System and Database for Life Cycle Engineering (GaBi) was 3.10 Comparability
used. All background data records relevant for production and Basically, a comparison or an evaluation of EPD data is only
disposal were almost exclusively taken from various GaBi possible if all the data sets to be compared were created
supplementary databases or rarely also from ecoinvent (v.3.6). according to EN 15804 and the building context, respectively
The data records included in the databases are documented the product-specific characteristics of performance, are taken
online. into account. The used background database is GaBi service
package 1 of 2023.
3.6 Data quality
4. LCA: Scenarios and additional technical information
The treatment of packaging as waste was modelled in Module
Characteristic product properties of biogenic carbon A5 as a weighted average.
The biogenic carbon content quantifies the amount of biogenic Modules B1-B7 are deemed not relevant since the product
carbon in a construction product leaving the factory gate, and it needs no maintenance or operational energy or water use and
is separately declared for the product and for any are therefore, not declared.
accompanying packaging.
Information on describing the biogenic Carbon Content at Installation into the building (A5)
factory gate The treatment of packaging as waste was modeled in Module
Name ValueUnit A5 as a weighted average. The following table depicts the
kg packaging materials treated in A5 with more than 1 gram of
Biogenic carbon content in product 0.016
C participation in the weighted average.
Modules B1-B7 are deemed not relevant since the product
Biogenic carbon content in accompanying kg
0.004 needs no maintenance or operational energy or water use and
packaging C
are, therefore, not declared.
Note: 1 kg of biogenic carbon is equivalent to 44/12 kg of CO .
2 Name Value Unit
Cardboard 0.010 kg
Pallet 0.004 kg
Polyethylene 0.001 kg
Transport to the building site (A4)
Name Value Unit Reference service life
Truck transport 27 t payload Name Value Unit
Transport distance 488 km Reference service life 10 a
Train transport 726 t payload
End of life (C1-C4)
Transport distance 12 km
Name Value Unit
Ship transport 27500 dwt payload
Incineration 97 %
Transport distance 272 km
Landfilling 3 %
Cargo plane transport 65 t payload
Transport distance 49 km For the calculation of this LCA landfilling is chosen for the US
and incineration for the EU. Different disposal routes are
Capacity utilisation (including empty runs) 80 - 90 %
available but not taken into account for this industry average
Because many different countries are involved, there were LCA.
always global data sets used to model the transport distances.
4 Environmental Product Declaration - IGI - The Global Wallcoverings Association - Vinyl wallcoverings on non-woven backing
Reuse, recovery and/or recycling potentials (D), relevant from thermal combustion of the wallcoverings are calculated in
scenario information Module D. From the total paper used as backing, 48.3% of
In module D the potential benefits of the thermal combustion of recycled paper in the product does not receive benefits, as it is
the wallcoverings (C3) and their packaging (A5) as well as the a secondary material coming burden-free to the system.
incineration of landfill gases (C4) are displayed. The benefits
5 Environmental Product Declaration - IGI - The Global Wallcoverings Association - Vinyl wallcoverings on non-woven backing
5. LCA: Results
In this section, the LCA results for 1 m² wallcoverings are presented. It should be borne in mind that the LCA results only indicate
possible effects.
Indicators used for evaluation:
The EN 15804+A2 LCIA methodology with the characterization factors infrom EU-JRC were used to evaluate the possible
environmental effects of the wallcoverings. The characterization factors are available at the following internet link:
http://eplca.jrc.ec.europa.eu/LCDN/developerEF.xhtml.
DESCRIPTION OF THE SYSTEM BOUNDARY (X = INCLUDED IN LCA; MND = MODULE OR INDICATOR NOT DECLARED; MNR
= MODULE NOT RELEVANT)
Benefits and
Construction loads beyond
Product stage Use stage End of life stage
process stage the system
boundaries
la ire ta m w a Ry lp p u s tro p s n a rT g n iru tc a fu n a M e h t m o rf tro p s n a rTe tis e h t o t e ta g y lb m e s s A e s U e c n a n e tn ia M ria p e R tn e m e c a lp e R tn e m h s ib ru fe R y g re n e la n o ita re p Oe s u re ta w la n o ita re p Oe s u n o itc u rts n o c -e Dn o itilo m e d tro p s n a rT g n is s e c o rp e ts a W la s o p s iD -e s u e R-y re v o c e R-g n ilc y c e Rla itn e to p
A1 A2 A3 A4 A5 B1 B2 B3 B4 B5 B6 B7 C1 C2 C3 C4 D
X X X X X MND MND MNR MNR MNR MND MND X X X X X
RESULTS OF THE LCA - ENVIRONMENTAL IMPACT according to EN 15804+A2: 1 m² vinyl wallcoverings on non-woven
backing
Parameter Unit A1-A3 A4 A5 C1 C2 C3 C4 D
GWP-total kg CO 2 eq 5.1E-01 4.72E-02 1.75E-02 2.66E-05 1.96E-03 3.28E-01 1.12E-03 -1.09E-01
GWP-fossil kg CO 2 eq 5.83E-01 4.71E-02 3.58E-03 2.66E-05 1.94E-03 2.71E-01 3.53E-04 -1.09E-01
GWP-biogenic kg CO 2 eq -7.22E-02 0 1.4E-02 0 0 5.74E-02 7.7E-04 0
GWP-luluc kg CO 2 eq -1.28E-03 8.99E-05 1.09E-06 8.89E-09 1.79E-05 1.53E-05 3.15E-07 -6.83E-06
ODP kg CFC11 eq 1.1E-09 3.72E-15 1.99E-15 1.62E-16 2.51E-16 1.6E-13 5.43E-16 -8.04E-13
AP mol H+ eq 1.54E-03 2.38E-04 5.28E-06 6.73E-08 1.61E-05 8.66E-05 1.18E-06 -1.31E-04
EP-freshwater kg P eq 1.51E-05 4.14E-08 2.95E-09 2.34E-09 7.06E-09 5.2E-08 5.94E-08 -1.66E-07
EP-marine kg N eq 4.19E-04 1.06E-04 2.01E-06 2.36E-08 8.05E-06 2.87E-05 3.54E-07 -3.87E-05
EP-terrestrial mol N eq 4.38E-03 1.16E-03 2.48E-05 1.63E-07 8.89E-05 3.84E-04 3.24E-06 -4.15E-04
kg NMVOC
POCP 1.4E-03 2.72E-04 5.05E-06 4.41E-08 1.52E-05 7.81E-05 1.17E-06 -1.08E-04
eq
ADPE kg Sb eq 8.59E-08 1.01E-09 2.53E-11 1.53E-12 1.27E-10 1.4E-09 1.01E-11 -7.41E-09
ADPF MJ 1.23E+01 6.36E-01 6.72E-03 4.75E-04 2.63E-02 3.42E-01 5.05E-03 -1.97E+00
m3 world eq
WDP 2.66E-01 1.75E-04 2.1E-03 8.59E-03 2.33E-05 3.72E-02 7.59E-07 -9.74E-03
deprived
GWP = Global warming potential; ODP = Depletion potential of the stratospheric ozone layer; AP = Acidification potential of land and water; EP =
Eutrophication potential; POCP = Formation potential of tropospheric ozone photochemical oxidants; ADPE = Abiotic depletion potential for non-fossil
resources; ADPF = Abiotic depletion potential for fossil resources; WDP = Water (user) deprivation potential)
RESULTS OF THE LCA - INDICATORS TO DESCRIBE RESOURCE USE according to EN 15804+A2: 1 m² vinyl wallcoverings on
non-woven backing
Parameter Unit A1-A3 A4 A5 C1 C2 C3 C4 D
PERE MJ 1.56E+00 1.15E-02 1.84E-01 9.67E-05 1.91E-03 9.12E-01 9.06E-03 -5.49E-01
PERM MJ 1.02E+00 0 -1.82E-01 0 0 -8.25E-01 -8.59E-03 0
PERT MJ 2.58E+00 1.15E-02 1.34E-03 9.67E-05 1.91E-03 8.68E-02 4.65E-04 -5.49E-01
PENRE MJ 9.19E+00 6.38E-01 4.83E-02 4.75E-04 2.64E-02 3.31E+00 1.01E-01 -1.97E+00
PENRM MJ 3.11E+00 0 -4.16E-02 0 0 -2.97E+00 -9.62E-02 0
PENRT MJ 1.23E+01 6.38E-01 6.72E-03 4.75E-04 2.64E-02 3.42E-01 5.05E-03 -1.97E+00
SM kg 3.36E-03 0 0 0 0 0 0 0
RSF MJ 0 0 0 0 0 0 0 0
NRSF MJ 0 0 0 0 0 0 0 0
FW m3 6.83E-03 1.3E-05 4.95E-05 2E-04 2.1E-06 9.06E-04 1.84E-07 -4.45E-04
PERE = Use of renewable primary energy excluding renewable primary energy resources used as raw materials; PERM = Use of renewable primary
energy resources used as raw materials; PERT = Total use of renewable primary energy resources; PENRE = Use of non-renewable primary energy
excluding non-renewable primary energy resources used as raw materials; PENRM = Use of non-renewable primary energy resources used as raw
materials; PENRT = Total use of non-renewable primary energy resources; SM = Use of secondary material; RSF = Use of renewable secondary fuels;
NRSF = Use of non-renewable secondary fuels; FW = Use of net fresh water
RESULTS OF THE LCA – WASTE CATEGORIES AND OUTPUT FLOWS according to EN 15804+A2:
1 m² vinyl wallcoverings on non-woven backing
Parameter Unit A1-A3 A4 A5 C1 C2 C3 C4 D
HWD kg 2.41E-05 1.35E-12 1.78E-13 1.35E-14 8.17E-14 2.14E-12 4.3E-13 -1.15E-10
NHWD kg 4.57E-02 6.58E-05 6.6E-04 6.08E-05 4.02E-06 8.44E-02 5.63E-03 -9.54E-04
6 Environmental Product Declaration - IGI - The Global Wallcoverings Association - Vinyl wallcoverings on non-woven backing
RWD kg 1.99E-04 7.76E-07 2.73E-07 1.9E-08 4.94E-08 1.24E-05 5.95E-08 -1.46E-04
CRU kg 0 0 0 0 0 0 0 0
MFR kg 0 0 0 0 0 0 0 0
MER kg 2.51E-02 0 1.13E-02 0 0 1.78E-01 0 0
EEE MJ 5.47E-02 0 0 0 0 0 0 4.84E-01
EET MJ 1.03E-01 0 0 0 0 0 0 9.5E-01
HWD = Hazardous waste disposed; NHWD = Non-hazardous waste disposed; RWD = Radioactive waste disposed; CRU = Components for re-use;
MFR = Materials for recycling; MER = Materials for energy recovery; EEE = Exported electrical energy; EET = Exported thermal energy
RESULTS OF THE LCA – additional impact categories according to EN 15804+A2-optional:
1 m² vinyl wallcoverings on non-woven backing
Parameter Unit A1-A3 A4 A5 C1 C2 C3 C4 D
Disease
PM 2.06E-08 1.1E-09 3.1E-11 1.08E-12 1.15E-10 1.18E-09 1.17E-11 -1.11E-09
incidence
IR kBq U235 eq 1.42E-01 1.11E-04 4.33E-05 2.91E-06 7.36E-06 1.66E-03 8.69E-06 -2.42E-02
ETP-fw CTUe 7.74E+00 4.47E-01 3.62E-03 9.77E-04 1.87E-02 1.96E-01 4.72E-03 -4.13E-01
HTP-c CTUh 8.1E-10 8.41E-12 1.75E-13 1.86E-14 3.85E-13 9.22E-12 2.29E-13 -2.15E-11
HTP-nc CTUh 8.14E-08 4.61E-10 8.43E-12 1.74E-12 2.33E-11 8.01E-10 2.06E-11 -6.77E-10
SQP SQP 4.42E+00 5.63E-02 2.09E-03 7.06E-05 1.1E-02 8.09E-02 4.63E-04 -3.61E-01
PM = Potential incidence of disease due to PM emissions; IR = Potential Human exposure efficiency relative to U235; ETP-fw = Potential comparative
Toxic Unit for ecosystems; HTP-c = Potential comparative Toxic Unit for humans (cancerogenic); HTP-nc = Potential comparative Toxic Unit for humans
(not cancerogenic); SQP = Potential soil quality index
Disclaimer 1 – for the indicator “Potential Human exposure efficiency relative to U235”. This impact category deals mainly with the
eventual impact of low-dose ionizing radiation on human health of the nuclear fuel cycle. It does not consider effects due to possible
nuclear accidents, occupational exposure or radioactive waste disposal in underground facilities. Potential ionizing radiation from the
soil, radon and from some construction materials is also not measured by this indicator.
Disclaimer 2 – for the indicators “abiotic depletion potential for non-fossil resources”, “abiotic depletion potential for fossil resources”,
“water (user) deprivation potential, deprivation-weighted water consumption”, “potential comparative toxic unit for ecosystems”,
“potential comparative toxic unit for humans – cancerogenic”, “Potential comparative toxic unit for humans - not cancerogenic”,
“potential soil quality index”. The results of this environmental impact indicator shall be used with care as the uncertainties on these
results are high as there is limited experience with the indicator.
This EPD was created using a software tool.
6. LCA: Interpretation
7 Environmental Product Declaration - IGI - The Global Wallcoverings Association - Vinyl wallcoverings on non-woven backing
demands. In the GWP category, the biogenic carbon dioxide
The production stage (module A1-A3) clearly dominates the contained in the paper is treated first as a credit; after
LCA results. The loads caused by the disposal stage (modules incineration in a waste-to-energy facility, it is treated as a load
C3 and C4) become noticeable, especially as the biogenic (C3). Moreover, paper production has a relatively large
carbon leaves the product system, reflected in the total and influence on the acidification potential (AP), the eutrophication
biogenic global warming potential. Transports play a potential (EP), the ozone depletion (ODP), and the Potential for
subordinate yet not insignificant role. the formation of tropospheric ozone (POCP).
The main environmental impacts are in all categories located in Transport processes do also affect GWP-fossil, AP, EP, POCP,
module A1-A3. For GWP-fossil and ADPF the highest precursor and ADPF. The main reason is the combustion of fuels.
of impact is the use of PVC plastisol for vinyl coating. The The waste treatment in module C3 in the GWP-fossil impact is
production and use of thermal and electric energy for general dominated by the incineration of PVC plastisol at End-of-Life.
production and heating/drying processes in A3 is the second-
highest precursor in both categories. The production of Range of the results
Titanium dioxide (TiO2) pigment and Di-isononyl phthalate The individual results of the participating companies differ from
(DINP) are substantial sources of GWP-fossil and ADPF. the average results in the present environmental product
The highest source of environmental impact in most categories declaration. Regarding GWP, the results may be 245% higher
is the production of PVC plastisol, not only because it or 41% lower than the average for this EPD.
constitutes 33% of the product mass; but because of the The main reason for the deviations is differences in the
energy-intensive production of PVC itself. grammage of the individual wallcoverings. In addition, there are
The production of paper has a noticeable effect. It has a different materials used as well as varying heat and electricity
relatively high share of the greenhouse potential due to energy consumptions depending on the manufacturer.
7. Requisite evidence
Members of the The Global Wallcoverings Association have the wallcoverings meet the requirements of test standard
following certificates: ISO 16000.
• Optional compliance with German RAL-GZ 479.
• The declared products comply with EN 15102.
• Optional compliance with USA Wallcovering Association
• According to the (emission) test chamber assessment,
W-101 (2013) paragraph 8.1 when tested by California
which follows to the French measurement method
Specification Section 01350 to criteria CDPH/EHLB
Arrêté du 19/04/11 the wallcoverings meet the
Standard Method V1.1 (2010).
requirements of the test standard ISO 16000.
The certificates and classifications for the various wallcoverings
• Optional according to the chamber test which follows
can be obtained from the respective manufacturers.
the German AgBB (Committee for health-related
evaluation of building products) regulations the
8. References
Standards and Norms
EN 12149:1997
Arrêté du 19/04/11 Wallcoverings in roll form - Determination of migration of heavy
Order of 19 April 2011 relating to the labeling of construction metals and certain other elements, of vinyl chloride monomer
products or wall or floor coverings and paints and varnishes on and of formaldehyde release.
their emissions of volatile pollutants
EN 12956:1999
ASTM E 84 Wallcoverings in roll form - Determination of dimensions,
ASTM E 84:2016: Standard Test Method for Surface Burning straightness, spongeability and washability.
Characteristics of Building Materials
EN 13501-1:2018
ASTM F 793 Fire classification of construction products and building
ASTM F793 / F793M-15, Standard Classification of Wall elements - Part 1: Classification using data from reaction to fire
Coverings by Use Characteristics, ASTM International, West Tests.
Conshohocken, PA, 2015
EN 15102:2007+A1:2011
ASTM F1141 - 93 Decorative wallcoverings - Roll and panel form.
ASTM F1141-93(2009), Standard Specification for
Wallcovering, ASTM International, West Conshohocken, PA, EN 233:2016
2009 Wallcoverings in roll form - Specification for finished wallpapers,
wall vinyls and plastics wallcoverings.
BNB
Lifetimes of components for life cycle analyses according to the EN 234:2019
Bewertungssystem Nachhaltiges Bauen, 2011. Wallcoverings in roll form – Specification for wallcoverings for
subsequent decoration
CDPH/EHLB
Standard method for measuring and evaluating chemical EN 235:2001
emissions from indoor sources using environmental chambers, Wallcoverings - Vocabulary and Symbols.
Version 1.1
EN 259-1:2001
CPR Wallcoverings in roll form - Heavy duty wallcoverings - Part 1:
Construction Product Regulation EU Specifications.
8 Environmental Product Declaration - IGI - The Global Wallcoverings Association - Vinyl wallcoverings on non-woven backing
of the European Parliament and of the Council of 9 March 2011
EN ISO 105-B02 laying down harmonised conditions for the marketing of
Textiles - Tests for colour fastness - Part B02: Colour fastness construction products and repealing Council Directive
to artificial light: Xenon arc fading lamp test (ISO 105- 89/106/EEC Text with EEA relevance. Current consolidated
B02:2014). version: 16/07/2021
EN ISO 14025:2006 WA-101
Environmental labels and declarations — Type III WA Quality Standard for Polymer Coated Fabric Wallcovering
environmental declarations — Principles and procedures; 2009-
11.
Further documentation
EN ISO 14044:2006
Environmental management - Life cycle assessment - Ecoinvent
Requirements and guidelines (ISO 14044:2006). Database for Life Cycle Assessment, version 3.6. Swiss Center
for Life Cycle Inventories, St. Gallen, 2023.
EN ISO 16000:2006
Indoor air - Part 3: Determination of formaldehyde and other European Commission
carbonyl compounds in indoor air and test chamber air - Active List of substances banned for use in cosmetic products. CMR
sampling method. substances of category 1A, 1B or 2 under Commission
Indoor air - Part 6: Determination of volatile organic compounds Regulation (EC) No 790/2009. 01/12/2010. Updated
in indoor and test chamber air by active sampling on Tenax 01/07/2015.
TA® sorbent, thermal desorption and gas chromatography
using MS or MS-FID. European Parliament
Indoor air - Part 9: Determination of the emission of volatile Regulation (EU) no 528/2012 of the European Parliament and
organic compounds from building products and furnishing - of the council of 22 may 2012 concerning the making available
Emission test chamber method. on the market and use of biocidal products.
Indoor air - Part 11: Determination of the emission of volatile
organic compounds from building products and furnishing - European Waste Catalogue (EWC)
Sampling, storage of samples and preparation of test European Waste Catalogue / Ordinance on European List of
specimens. Wastes
ISO 14001:2015 EU-JRC
Environmental management systems - Requirements with EN 15804 reference package. Flows, Methods,
guidance for use. Characterisation Factors, Unit Groups and Flow Properties
based on EF Reference Package 3.0.
EN 15804
EN 15804:2012+A2:2019+AC:2021, Sustainability of German AgBB
construction works — Environmental Product Declarations — Committee for health-related evaluation of building products.
Core rules for the product category of construction products. Umweltbundesamt Deutschlands.
ISO 50001:2011 Institut Bauen und Umwelt e. V.
Energy management systems - Requirements with guidance for Product Category Rules for Building-Related Products and
use. Services – PCR-A: Part A+A2: Calculation Rules for the Life
Cycle Assessment and Requirements on the Project Report
SVHC according to EN 15804+A2:2019, version: 1.3 from 31/08/2022.
Candidate List of substances of very high concern for
Authorisation (SVHC) Institut Bauen und Umwelt e. V.
Published in accordance with Article 59(10) of the REACH PCR Guidance-Texts for Building-Related Products and
Regulation. European chemicals agency (ECHA). Services - Part B: Requirements on the EPD for Wallcoverings.
Version: 8 from 01/08/2021.
RAL-GZ 479
Wallpapers - Quality assurance LCA for Experts (GaBi)
LCA for Experts 10.7.0.183: Software System and Database for
Regulation (EU) No 305/2011 Life Cycle Engineering. 1992-2023. Sphera Solutions GmbH
9 Environmental Product Declaration - IGI - The Global Wallcoverings Association - Vinyl wallcoverings on non-woven backing
Publisher
Institut Bauen und Umwelt e.V. +49 (0)30 3087748- 0
Hegelplatz 1 info@ibu-epd.com
10117 Berlin www.ibu-epd.com
Germany
Programme holder
Institut Bauen und Umwelt e.V. +49 (0)30 3087748- 0
Hegelplatz 1 info@ibu-epd.com
10117 Berlin www.ibu-epd.com
Germany
Author of the Life Cycle Assessment
brands & values GmbH +49 421 70 90 84 33
Altenwall 14 info@brandsandvalues.com
28195 Bremen www.brandsandvalues.com
Germany
Owner of the Declaration
IGI - The Global Wallcoverings Association +32 (0) 2 720 00 09
Chaussée de Louvain 426 info@igiwallcoverings.org
1380 LASNE www.igiwallcoverings.org
Belgium
10 Environmental Product Declaration - IGI - The Global Wallcoverings Association - Vinyl wallcoverings on non-woven backing
