ENVIRONMENTAL PRODUCT DECLARATION
as per ISO 14025 and EN 15804+A1
Owner of the Declaration ArcelorMittal Brasil
Programme holder Institut Bauen und Umwelt e.V. (IBU)
Publisher Institut Bauen und Umwelt e.V. (IBU)
Declaration number EPD-ARC-20190174-CBC2-EN
Issue date 09.03.2020
Valid to 08.03.2025
Hot Dip Coated Steel with Galvalume®
ArcelorMittal Brasil
www.ibu-epd.com | https://epd-online.com
Umwelt Produktdeklaration Name des Herstellers – Name des Produkts
General Information
ArcelorMittal Brasil Hot Dip Coated Steel with Galvalume®
Programme holder Owner of the declaration
IBU – Institut Bauen und Umwelt e.V. ArcelorMittal Brasil
Panoramastr. 1 Av. Carandaí, 1115
10178 Berlin 30130-915 - Belo Horizonte - MG
Germany Brazil
Declaration number Declared product / declared unit
EPD-ARC-20190174-CBC2-EN The declared unit is 1 metric ton of Galvalume® coated
steel produced by ArcelorMittal in Brazil (1mm steel
thickness with 3.8g/cm3 Galvalume® coating)
This declaration is based on the product Scope:
category rules: This declaration and its LCA study are relevant to 1
Structural steels, 07.2014 metric ton of Galvalume® steel manufactured by
(PCR checked and approved by the SVR) ArcelorMittal Brasil, representing 100% of the
production in 2017.
Issue date
09.03.2020 The owner of the declaration shall be liable for the
underlying information and evidence; the IBU shall not
be liable with respect to manufacturer information, life
Valid to
cycle assessment data and evidences.
08.03.2025
The EPD was created according to the specifications
of EN 15804+A1. In the following, the standard will be
simplified as EN 15804.
Verification
The standard EN 15804 serves as the core PCR
Independent verification of the declaration and data
according to ISO 14025:2010
Dipl. Ing. Hans Peters internally x externally
(chairman of Institut Bauen und Umwelt e.V.)
Dr. Alexander Röder Dr.-Ing. Wolfram Trinius
(Managing Director Institut Bauen und Umwelt e.V.)) (Independent verifier appointed by SVR)
Product
Product description/Product definition
This Environmental Product Declaration refers to a Application
double-sided hot dip galvanized coated steel, Tiles and thermoacoustic panels for roofs and facades,
consisting of steel substrate with a specific metallic flashings and gutters, profiles for light steel framing
alloyed zinc coating, Galvalume®, applied by means of and silos. Additionally, applications in white line and in
a continuous hot dip galvanising process. the agricultural and machinery segments, etc.
The Galvalume® basic composition is: 55% aluminum, Other applications are also possible in other market
43.4% zinc and 1.6% silicon. The combined action of segments.
the aluminum and the zinc gives extraordinary
corrosion resistance to this type of coating, where the Technical Data
first creates a protection barrier whilst the latter
becomes the sacrificing element providing galvanic
protection. Among its most important characteristics Name Value Unit
are high reflectivity, which generates higher thermal Density 7825 kg/m³
efficiency, and high heat resistance with no loss of Thermal conductivity 48 W/(mK)
protection, brilliance and colouring characteristics. Modulus of elasticity 210000 N/mm²
Coefficient of thermal expansion 12 10-6K-1
Galvalume® coated steels are described according to Melting point 1536 °C
NBR 15578. They are available in a very wide range of
steel grades and coating density of 3.8 g/cm3.
Performance data of the product with respect to its
For the use and application of the product the characteristics in accordance with the relevant
respective national provisions at the place of use technical provision (no CE-marking).
apply.
2 Environmental Product Declaration ArcelorMittal Brasil – Galvalume
Base materials/Ancillary materials https://brasil.arcelormittal.com/produtos-
The base material of aluminum and zinc coated steel solucoes/catalogos
is iron.
Reference service life
Alloying elements are added on the form of ferroalloys
or metals. The metallic coating includes aluminum and Reference service life is not relevant due to cradle-to-
zinc. gate with options (C3 and D) boundary conditions.
Detailed information about mechanical properties and
coatings are available at:
LCA: Calculation rules
Declared Unit waste status once is shredded and sorted,
thus becomes input to the product system in
The declaration refers to the functional unit of 1 metric
the inventory.
ton of Galvalume® coated steel as specified in Part
B requirements on the EPD for Structural Steel.
Declared unit Module C3 takes into account the sorting and
Name Value Unit shredding of after-use steel, as well as the non-
Declared unit 1 t recovered scrap due to sorting efficiency which is
Thickness (of sheet) 1 mm landfilled. A conservative value of 2% landfill is
Coating density 3.8 g/cm³ considered.
Conversion factor to 1 kg 0.001 -
Module D refers to the net benefits and loads of the
net flow leaving the product system.
System boundary
Data Quality
The study is performed from ‘cradle-to-gate’ + module
The life cycle inventory data used in this study comply
C3 and module D (cradle to gate - with Options). The
with the quality requirements set out in ISO 14044.
following life cycle stages are considered:
 Product stage
All relevant background datasets are taken from GaBI
 End-of-life through Waste processing
ts Software database - Service Pack 37 and comprise
 Benefits and loads beyond the product the year 2018. Such database contains consistent and
system boundary documented datasets which can be viewed in the
online GaBI ts documentation.
Modules A1-A3 include the following:
Regarding foreground data, this study is based on a
high quality of primary data for the year 2017, collected
 The provision of resources, additives and
by ArcelorMittal.
energy;
 Transport of resources additives to the Comparability
production site Basically, a comparison or an evaluation of EPD data
 Production processes on site including is only possible if all the data sets to be compared
were created according to EN 15804 and the building
energy, production of additives, disposal of
context, respectively the product-specific
production residues, and consideration of
characteristics of performance, are taken into account.
related emissions;
 Recycling of production/manufacturing scrap. .
Steel scrap is assumed to reach the end-of-
LCA: Scenarios and additional technical information
Name Value Unit
End of life (C3)
Landfilling 10 kg
Due to the absence of official national references and
recommendation of the Brazilian context, Recycling
and Reuse rates adopted for this EPD were defined
Reuse, recovery and/or recycling potentials (D),
according to the recommendations of European
relevant scenario information
Commission Technical Steel Research for “Other
18,6 kg scrap is used in the manufacturing of 1 ton of
steel”: 99% (Recycling and Reuse) and 1% (Landfill).
Galvalume steel. After use, 990 kg steel is recycled.
Such assumptions are similar to current practices and
The potential environmental benefit calculated for the
rates in the Brazilian market, which would not result in
end-of-life stage (module D) is based on the net
visible changes of the EPD results.
amount of scrap in the system: 990 – 18,6 = 971 kg.
3 Environmental Product Declaration ArcelorMittal Brasil – Galvalume
The system net output carries a potential credit, thus
module D shows an environmental benefit.
Name Value Unit
Reuse 11 %
Recycling 88 %
Landfill 1 %
4 Environmental Product Declaration ArcelorMittal Brasil – Galvalume
LCA: Results
DESCRIPTION OF THE SYSTEM BOUNDARY (X = INCLUDED IN LCA; MND = MODULE NOT DECLARED;
MNR = MODULE NOT RELEVANT)
BENEFITS AND
CONSTRUCTI LOADS
PRODUCT STAGE ON PROCESS USE STAGE END OF LIFE STAGE BEYOND THE
STAGE SYSTEM
BOUNDARIES
5 Environmental Product Declaration ArcelorMittal Brasil – Galvalume
lairetam
waR
ylppus tropsnarT
gnirutcafunaM
eht
morf
tropsnarT
etis
eht
ot
etag
ylbmessA esU
ecnanetniaM
riapeR
tnemecalpeR tnemhsibrufeR
ygrene
lanoitarepO esu
retaw
lanoitarepO esu
noitcurtsnoc-eD
noitilomed tropsnarT
gnissecorp
etsaW
lasopsiD -esueR -yrevoceR -gnilcyceR laitnetop
A1 A2 A3 A4 A5 B1 B2 B3 B4 B5 B6 B7 C1 C2 C3 C4 D
X X X MND MND MND MND MNR MNR MNR MND MND MND MND X MND X
RESULTS OF THE LCA - ENVIRONMENTAL IMPACT according to EN 15804+A1: 1 t Galvalume®
Parameter Unit A1-A3 C3 D
Global warming potential [kg CO2-Eq.] 2.60E+3 2.54E+1 -1.56E+3
Depletion potential of the stratospheric ozone layer [kg CFC11-Eq.] 2.30E-5 3.14E-6 8.71E-6
Acidification potential of land and water [kg SO2-Eq.] 1.30E+1 2.30E-1 -3.08E+0
Eutrophication potential [kg (PO4)3--Eq.] 1.66E+0 1.04E-1 -2.28E-1
Formation potential of tropospheric ozone photochemical
[kg ethene-Eq.] 1.33E+0 1.77E-2 -7.21E-1
oxidants
Abiotic depletion potential for non-fossil resources [kg Sb-Eq.] 1.01E-2 4.61E-4 -4.79E-3
Abiotic depletion potential for fossil resources [MJ] 2.48E+4 3.55E+2 -1.52E+4
RESULTS OF THE LCA - RESOURCE USE according to EN 15804+A1: 1 t Galvalume®
Parameter Unit A1-A3 C3 D
Renewable primary energy as energy carrier [MJ] 1.39E+3 5.40E+1 1.00E+3
Renewable primary energy resources as material utilization [MJ] 0.00E+0 0.00E+0 0.00E+0
Total use of renewable primary energy resources [MJ] 1.39E+3 5.40E+1 1.00E+3
Non-renewable primary energy as energy carrier [MJ] 2.52E+4 4.06E+2 -1.46E+4
Non-renewable primary energy as material utilization [MJ] 0.00E+0 0.00E+0 0.00E+0
Total use of non-renewable primary energy resources [MJ] 2.52E+4 4.06E+2 -1.46E+4
Use of secondary material [kg] 1.86E+1 0.00E+0 9.71E+2
Use of renewable secondary fuels [MJ] -2.03E-30 0.00E+0 0.00E+0
Use of non-renewable secondary fuels [MJ] -2.40E-29 0.00E+0 0.00E+0
Use of net fresh water [m³] 6.90E+0 1.83E-1 2.10E+0
RESULTS OF THE LCA – OUTPUT FLOWS AND WASTE CATEGORIES according to EN 15804+A1:
1 t Galvalume®
Parameter Unit A1-A3 C3 D
Hazardous waste disposed [kg] 2.91E-4 3.84E-8 -1.02E-3
Non-hazardous waste disposed [kg] 7.94E+2 1.00E+1 1.68E+2
Radioactive waste disposed [kg] 7.69E-2 9.68E-5 5.02E-4
Components for re-use [kg] 0.00E+0 0.00E+0 0.00E+0
Materials for recycling [kg] 0.00E+0 9.90E+2 0.00E+0
Materials for energy recovery [kg] 0.00E+0 0.00E+0 0.00E+0
Exported electrical energy [MJ] 0.00E+0 0.00E+0 0.00E+0
Exported thermal energy [MJ] 0.00E+0 0.00E+0 0.00E+0
Interpretation
The production stage is the high contributing stage in the life cycle of Galvalume®.
Module C3 has a low contribution while module D presents negative contribution (credit) for all impact categories
except ODP.
Due to the Hot-Rolled Steel Coil input, the Pickling stage is the biggest contributor in all environmental categories
except ADPE, in which Galvanization is the process that presents the highest contribution due to the zinc and
aluminium coating.
Module D has a significant part for the results, especially for GWP and ADPE (expressive only in Hot-Rolled Steel
Coil).
This is because the external scrap input is low, which increase the net scrap value, reducing the original impact of
the production (A1-A3).
Total use of renewable primary energy carrier (PERT) and total use of non-renewable primary energy (PENRT)
are dominated by the extraction and processing of raw materials and the generation of electricity, steam and heat
from primary energy resources, including extraction, refining and transport.
In general, the main contribution to primary energy in the blast furnace/basic oxygen furnace (BF/BOF) route
comes from the use of coal/coke as an energy and carbon source.
References
PCR part A
Product Category Rules for Construction Products. Worldsteel 2014
Part A: Calculation Rules for the Life Cycle Worldsteel 2014: A methodology to determine the LCI
Assessment and Requirements on the Background of steel industry co-products.
Report. Berlin: Institut Bauen und Umwelt e.V. (IBU), https://www.worldsteel.org/en/dam/jcr:167ec6bc-d974-
2013. 4405-8d53-56825ad4552f/Co-
product+methodology+for+the+steel+industry+2014.pd
PCR part B f
Product Category Rules for Construction Products.
Part B: Requirements on the EPD for Structural Steels. NBR 15578
Berlin: Institut Bauen und Umwelt e.V. (IBU), 2014. ABNT NBR 15578:2008, Continuous hot-dip 55%
aluminum-zinc coated steels strip and sheet -
ArcelorMittal Vega, 2019. Available online: Specification
https://brasil.arcelormittal.com/a-arcelormittal/quem-
somos/arcelormittal-vega ISO 14040
DIN EN ISO 14040:2009-11, Environmental
European Commission Technical Steel Research, management - Life cycle assessment - Principles and
Sansom, M. and Meijer, J.: Life-cycle assessment framework
(LCA) for steel construction, 2001-12
ISO 14044
Gabi ts Software DIN EN ISO 14044:2006-10, Environmental
GaBi 8.7. Software System and Holistic Accounting management - Life cycle assessment - Requirements
Database, Version 8.7.0.18. Stuttgart, Echterdingen: and guidelines
thinkstep AG, Service Package/SP 37 [accessed
01.10.2019]. EN 15804
EN 15804:2012-04+A1 2013/, Sustainability of
GaBi ts Documentation construction works — Environmental Product
Documentation of the GaBi datasets for Life Cycle Declarations — Core rules for the product category of
Engineering. LBP, Universitity of Stuttgart and PE construction products
International, 2017. http://documentation.gabi-
software.com
6 Environmental Product Declaration ArcelorMittal Brasil – Galvalume
Publisher
Institut Bauen und Umwelt e.V. Tel +49 (0)30 3087748- 0
Panoramastr. 1 Fax +49 (0)30 3087748- 29
10178 Berlin Mail info@ibu-epd.com
Germany Web www.ibu-epd.com
Programme holder
Institut Bauen und Umwelt e.V. Tel +49 (0)30 - 3087748- 0
Panoramastr 1 Fax +49 (0)30 – 3087748 - 29
10178 Berlin Mail info@ibu-epd.com
Germany Web www.ibu-epd.com
Author of the Life Cycle
Assessment Tel +55 (11) 2349-3006
Espaço Eco Foundation Fax 0
Estrada Ribeirão do Soldado 230 Mail espacoeco@basf.com
982201 São Bernardo do Campo, Web www.espacoeco.org.br/
SP – Brasil
Brazil
Owner of the Declaration
ArcelorMittal Brasil Tel 0800 015 1221
Av. Carandaí, 1115 - Funcionários Fax -
25 an Mail
30130 -915 - Belo Horizonte arcelormittalnet@arcelormittal.co
Brazil m.br
Web
http://www.arcelormittal.com.b
r/
