ENVIRONMENTAL PRODUCT DECLARATION
as per ISO 14025 and EN 15804+A2
Owner of the Declaration VELUX Group
Publisher Institut Bauen und Umwelt e.V. (IBU)
Programme holder Institut Bauen und Umwelt e.V. (IBU)
Declaration number EPD-VEL-20220139-IBJ3-EN
Issue date 25.07.2022
Valid to 24.07.2027
VELUX flat roof window CXP
VELUX A/S
www.ibu-epd.com | https://epd-online.com
1. General Information
VELUX A/S VELUX flat roof window CXP
Programme holder Owner of the declaration
IBU – Institut Bauen und Umwelt e.V. VELUX Group
Hegelplatz 1 Ådalsvej 99
10117 Berlin 2970 Hørsholm
Germany Denmark
Declaration number Declared product / declared unit
EPD-VEL-20220139-IBJ3-EN The declaration represents 1 piece of a VELUX flat roof window CXP of
the size 1.20 m x 1.20 m = 1.44 m2
This declaration is based on the product category rules: Scope:
Windows and doors , 01.08.2021 The declaration covers 100% of VELUX flat roof windows CXP by
(PCR checked and approved by the SVR) Partizánske Building Components SK, Slovenia.
The owner of the declaration shall be liable for the underlying information
and evidence; the IBU shall not be liable with respect to manufacturer
Issue date information, life cycle assessment data and evidences.
25.07.2022
The EPD was created according to the specifications of EN 15804+A2. In
the following, the standard will be simplified as EN 15804.
Valid to
Verification
24.07.2027
The standard EN 15804 serves as the core PCR
Independent verification of the declaration and data according to ISO
14025:2011
internally X externally
Dipl.-Ing. Hans Peters
(Chairman of Institut Bauen und Umwelt e.V.)
Florian Pronold Dr. Eva Schmincke,
(Managing Director Institut Bauen und Umwelt e.V.) (Independent verifier)
1 Environmental Product Declaration - VELUX A/S - VELUX flat roof window CXP
2. Product
galvanized steel 15 %
2.1 Product description/Product definition laminated glass 25 %
The Velux Flat roof windows CXP consists of a manually tempered glass 10 %
operated base unit made of a PVC curb with an integrated others
glazing unit and hinges on one side to allow for venting and a
top unit with one-layer opaque or transparent acrylic (PMMA) Composition of the top unit (ISD 0000A):
dome. For the placing on the market of the product in the PMMA 95 %
European Union/European Free Trade Association (EU/EFTA) iron & cast iron 5 %
(with the exception of Switzerland) Regulation (EU) No.
305/2011 (CPR) applies. The product needs a declaration of 1) 'This product/article/at least one partial article contains
performance taking into consideration EN 1873:2005, substances listed in the candidate list (date: 02.03.2022)
Prefabricated accessories for roofing - Individual rooflights of exceeding 0.1 percentage by mass:
plastics - Product specification and test methods and the CE-
• no
marking. For the application and use the respective national
2) 'This product/article/at least one partial article contains other
provisions apply.
CMR substances in categories 1A or 1B which are not on the
2.2 Application candidate list, exceeding 0.1 percentage by mass:
Velux flat roof windows CXP are used in renovation and new • not investigated with suppliers
build. 3) 'Biocide products were added to this construction product or
it has been treated with biocide products (this then concerns a
2.3 Technical Data treated product as defined by the (EU) Regulation on Biocidal
The Declaration of Performance including relevant technical Products No. 528/2012):
specifications and test methods/test standards can be
• no
downloaded from the website www.velux.com/ce.
Recycled content
The declared values in the table relate to the reference product
incl. an average pane. For other covered product variants,
specific values can be selected at the bottom of the above-
mentioned download page
Constructional data for CXP 120120 73Q+ISD 0000
For other variants, see velux.com/ce
Name Value Unit The values stated in the table relate to the recycled material
streams in VELUX production.
Reaction to fire - class
Resistance to upward load EN 1875 UL 1500 -
water permeability acc. to EN 13985, EN 2.6 Manufacture
- class
1027 Base unit:
Resistance to downward load EN 1873 UL 2500 -
Resistance to fire EN 13501-2 NPD - PVC profiles, gaskets and other minor components are
produced outside Velux.
External fire performance EN 13501-5 NPD -
Water tightness EN 1873 passed -
The insulating glass unit is assembled at a production site in
Impact resistance - small hard body passed France.
passed -
EN 1873
Impact resistance - large soft body EN 1873 SB 1200 - Minor ABS plastic and glass fibre components are produced at
Direct airborne sound insulation EN ISO 36 (-1;- a factory in Denmark.
dB
410-3 4)
The production and final assembly of the base unit takes place
Thermal transmittance EN 1873 0,86 W/(m2K)
at the production site in Slovakia.
Luminous transmittance EN 410 0,72 -
Air permability EN 1026 4 Class The final production processes includes preparation of the PVC
Durability EN 1873 NPD - frame/sash profiles by cutting, milling and drilling and
installation of EPS foam. The final PVC base is assembled by
Performance data of the product in accordance with the
cutting, deburring and welding, cutting and mounting of gaskets
declaration of performance with respect to its essential
and installation of the glazing unit, as well as packaging,
characteristics according to
stacking and wrapping of the product on pallets.
• EN 1873:2005, Prefabricated accessories for roofing -
Individual rooflights of plastics - Product specification Top unit:
and test methods
The plastic dome is produced and assembled at a production
2.4 Delivery status
site in Germany.
The product is available in pre-defined sizes covering 0,6x0,6m
to 1,5x1,5m.
The final production processes include forming/blow moulding
of the plastic dome, with afterwards deburring, engraving and
2.5 Base materials/Ancillary materials
assembly, as well as packaging, stacking and wrapping of the
Composition of the base unit CXP:
product on pallets.
PVC 40 %
2 Environmental Product Declaration - VELUX A/S - VELUX flat roof window CXP
The factories are ISO 9001 certified. Fire
2.7 Environment and health during manufacturing
Fire performance according to EN 13501:1
All factories are ISO 14001 and ISO 45001 certified.
Name Value
2.8 Product processing/Installation
Building material class B
The product is delivered to the customer in two parts, a top and
Burning droplets s1
bottom part. After the hole in the roof is prepared, the bottom
Smoke gas development d0
part of the product can be installed with the use of a
screwdriver, after which the top unit can be fastened to the
bottom unit. Water
In the event of unforeseen exposure to water (flood), no
2.9 Packaging
adverse effects on human health or the environment are to be
The packaging usually consists of: expected.
- polyethylene film
- polystyrene foam parts Mechanical destruction
- cardboard In the event of unforeseen mechanical destruction, VELUX flat
roof windows must be replaced; apart from potential injuries
The use of other packaging materials is possible, but from glass cullet, no adverse effects on human health or the
insignificant in terms of quantity. environment are to be expected.
The plastic packaging (polyethylene (PE) film, polystyrene foam 2.14 Re-use phase
parts) can be recycled if separated by type; alternatively, they VELUX flat roof windows can be dismantled manually without
can be incinerated. any problems. The metal parts are usually recycled, and the
plastic parts and wood are sent for thermal recycling for energy
2.10 Condition of use
recovery. Flat glass can be recycled whereas laminated glass is
The material composition of VELUX flat roof windows does not usually used as secondary aggregate in road construction or
change over their service life. landfilling.
2.11 Environment and health during use 2.15 Disposal
VELUX flat roof windows do not contain any pollutants that VELUX flat roof windows are mostly inert and can be disposed
could be released during use. of in an appropriate landfill. However, due to the value of the
materials or the carbon content of the plastic parts and wood,
Environmental protection: According to current knowledge, recycling or energy recovery is preferable and common.
hazards to water, air and soil cannot arise when the products
are used as intended. Waste code according to the European Waste List (Regulation
on the European Waste List):
Health protection: According to current knowledge, no health
hazards or impairments are to be expected. 17 02 02 glass
17 02 03 plastics
2.12 Reference service life
17 04 14 mixed metals
It is not possible to calculate the reference service life
according to ISO 15686. The service life based on a 2.16 Further information
manufacturer's declaration is 30 years. The corresponding Further documentation on the products, technical data sheets,
utilization scenario is declared in 4. BIM files, etc. can be found at:
www.velux.com
2.13 Extraordinary effects
3. LCA: Calculation rules
accordance with COUNCIL REGULATION (EU) No 333/2011,
3.1 Declared Unit secondary metals are modeled as part of the product system
The declared unit is 1 piece of a manually operated VELUX flat from the moment they are available as unmixed scrap.
roof window CXP with a base unit made of a PVC curb with an Waste or secondary fuels are not used for production.
integrated glazing unit with 1.20 m x 1.20 m = 1.44 m2.
Module A4 is not declared due to large variances in transport
Declared unit
distances between the production site and the construction site,
Name Value Unit
where the product is installed.
Declared unit 1 piece
Area 1.44 m2 Module A5: The products are delivered to the construction site
Weight 88,1 kg ready to be installed. Manual installation is assumed; electricity
consumption related to electric drilling machines, screw drivers,
etc. is considered to be negligible. The combustible packaging
material (plastics, wood, etc.) is assumed to be thermally
3.2 System boundary
treated in a municipal waste incineration plant with an efficiency
Type of EPD: Cradle to gate with options, with modules C1 –
R1 < 0.6 (according to the ecoinvent dataset used); the
C4, and module D (A1-A3, C1-C3, D and additional modules
recovered energy is declared as exported energy. Metals and
cardboard are recycled; it is assumed that these fractions reach
The production of VELUX flat roof windows (modules A1-A3)
the end-of-waste state after having been sorted and
includes raw material extraction, energy generation, waste
transported (as a conservative choice) to a recycler. No
treatment and all transports up to the factory gate. In
packaging waste is landfilled.
3 Environmental Product Declaration - VELUX A/S - VELUX flat roof window CXP
have been known to the project managers and would have
Modules B1 to B7 are not relevant for the product under contributed significantly to the indicators of the impact
consideration or no significant environmental impacts occur. assessment.
Module C1 includes manual dismantling, with no significant 3.5 Background data
environmental impact. Ecoinvent 3.8 (2021) is used as the background database.
3.6 Data quality
Module C2 comprises the transport of the dismantled VELUX
flat roof window to a sorting plant and then to a waste The foreground data are based on extensive and detailed data
incineration plant for the thermally treated plastic fraction. collection at the production site. The foreground data could be
fully linked with corresponding data records from the
Modules C3/C4: given the complexity of the inventoried background database ecoinvent 3.8.
products, a mixed end-of-life scenario is modelled, allowing the The background data was updated in 2021. Thus, the quality of
different materials to follow their most likely path. the foreground and background data can be rated as very
As a rule of thumb, metals are recycled and plastics are good.
incinerated (also due to the very limited data availability of
3.7 Period under review
plastics recycling and its benefits); coated and uncoated flat
The LCA data represents the production conditions for the year
glass is assumed to be recycled whereas laminated glass is
2021.
assumed to be landfilled due to very limited recycling potential.
Metals and flat glass recycled; it is assumed that these fractions 3.8 Geographic Representativeness
reach the end-of-waste state after having been sorted and
Land or region, in which the declared product system is
transported to a recycler; laminated glass is landfilled. The
manufactured, used or handled at the end of the product´s
combustible material (plastics, etc.) is assumed to be thermally
lifespan: Europe
treated in a municipal waste incineration plant.
Module D includes the benefits and burdens associated with 3.9 Allocation
recycling metals beyond the system boundary, resulting from No co-products are generated during the production of the
the treatment of recycled materials from the point of end-of- VELUX products. Sorted production scrap of the different
waste to the point of substitution (as loads) and substitution of metals, notably aluminium, is considered a secondary material
primary resources (as benefits). with no economic value (so no burdens allocated) and
It also includes the benefits and burdens associated with considered in the quantification of net flows leaving the product
energy recovery from plastic waste in a municipal waste system. This approach is chosen to ensure a coherent
incineration plant, as modeled in Module C3. quantification of net flows entering module D.
In Module D, only net flows of metals leaving the product
system are considered. No processes were modelled as part of the foreground model
that would have required an allocation of multi-input processes.
3.3 Estimates and assumptions
Background datasets on municipal waste incineration plants
No further assumptions and estimates relevant to the result had
were taken from ecoinvent without any modification.
to be made beyond the points made in this chapter 3 and in
chapter 4.
Allocation of reuse, recycling and recovery was avoided by the
cut-off approach in the foreground model in line with DIN EN
3.4 Cut-off criteria
15804.
No data available from the company survey was neglected.
These include, among other things, material use, energy 3.10 Comparability
demand (heat, electricity), packaging materials of raw materials
Basically, a comparison or an evaluation of EPD data is only
(insofar as they are generated as waste) and product
possible if all the data sets to be compared were created
packaging, consumables in production, waste treatment and
according to EN 15804 and the building context, respectively
the transport of all inputs and outputs.
the product-specific characteristics of performance, are taken
With this approach, mass and energy flows below 1 % were
into account.
also accounted for. No processes were neglected that would
4. LCA: Scenarios and additional technical information
Characteristic product properties of biogenic carbon Module A5
The products are delivered to the construction site ready to be
Information on describing the biogenic carbon content at installed. Manual installation is assumed, and electricity
factury gate consumption related to electric drilling machines, screw drivers,
etc. is considered to be negligible.
Name ValueUnit
The combustible packaging material (plastics, wood, etc.) is
kg
Biogenic carbon content in product 0.255 assumed to be transported 50 km with a lorry 16-32 metric
C
tons, EURO6 to an incineration plant with an efficiency R1 < 0.6
Biogenic carbon content in accompanying kg (according to the ecoinvent dataset used); the recovered
1.94
packaging C energy is declared as exported energy; for its quantification an
efficiency of 25.6 % is assumed for the production of heat and
Note: 1 kg of biogenic carbon is equivalent to 44/12 kg of CO .
2
13.0 % for the production of electricity (always referring to the
lower heating value of the waste).
Metals and cardboard are recycled; it is assumed that these
fractions reach the end-of-waste state after having been sorted
and transported (as a conservative choice) to a recycler over
4 Environmental Product Declaration - VELUX A/S - VELUX flat roof window CXP
150 km with a lorry 16-32 metric tons, EURO6. follow their most likely path.
No packaging waste is landfilled.
The use of multi-way pallets is not taken into account as It should also be noted that the deconstruction and waste
packaging material. treatment scenario can vary a lot, depending on the actual
situation. Thus, a generic end-of-life scenario is assumed.
Reference service life
Name Value Unit As a rule of thumb, metals are recycled, plastics are incinerated
(also due to the very limited availability on plastics recycling
Reference service life
and its benefits); coated and uncoated flat glass is assumed to
according to 30 a
be recycled whereas laminated glass is assumed to be
manufacturer's declaration
landfilled due to very limited recycling potential.
The product has passed
Declared product
internal quality controls and
properties (at the gate) and - The combustible material (mainly plastics) is assumed to be
complies with EN 1873 for CE
finishes transported 50 km with a lorry 16-32 metric tons, EURO6 to an
marking
incineration plant.
Design application
parameters (if instructed by Metals and flat glass recycled; it is assumed that these fractions
Installation according to
the manufacturer), reach the end-of-waste state after having been sorted and
assembly instructions and -
including the references to transported to a recycler over 150 km with a lorry 16-32 metric
state of the art.
the appropriate practices tons, EURO6.
and application codes
An assumed quality of Laminated glass is landfilled, including a transport of 30 km with
Carried out in accordance
work, when installed in a lorry 16-32 metric tons, EURO6.
with the manufacturer's -
accordance with the
instructions.
manufacturer’s instructions Module C3
Outdoor environment, (for The declared products are A consumption of 0.03 kWh/kg of electricity for shredding and
outdoor applications), e.g. intended for installation sorting and 0.437 MJ/kg of diesel fuel for internal logistics are
weathering, pollutants, UV outside the building: They are taken into account to disassemble the product. The recovered
and wind exposure, therefore designed to - material leaves the product system as 'materials for recycling'.
building orientation, withstand outdoor conditions The net amounts of the metals leaving the product system are
shading, temperature throughout their service life. considered as 'use of secondary material' in Module D.
Indoor environment (for
The declared products are Module C4
indoor applications), e.g.
not intended for installation - As stated above, it is assumed that 100 % of the plastic parts
temperature, moisture,
inside a building. and the wooden parts are treated in a waste incineration plant
chemical exposure
with an efficiency R1 < 0.6 (according to the ecoinvent dataset
Usage conditions, e.g. Standard use in any type of
used); 25.57 % of the lower heating value of the plastic parts
frequency of use, building, i.e. opening/closing -
are recovered as heat and 13.0 % as electricity. Recovered
mechanical exposure as often as necessary.
energy is reported as 'exported energy' and considered in
The declared products are Module D.
Maintenance e.g. required designed for a reference life
frequency, type and quality of 30 years. They are - Some of the material, notably laminated flat glass is assumed
and replacement of maintained by cleaning water to be landfilled.
components at the discretion of the
building occupants. Module D
Module B1 Module D contains the benefits and loads beyond the system
The products are assumed to have no direct emissions during boundary related to the recycling of metals, which result from
the use phase. The indicator values of Module B1 are thus 0. the treatment of recycled materials from the point of end-of-
For biogenic carbon storage, see table above. waste status to the point of substitution (as loads) and the
substitution of primary resources (as benefits).
Module B2
For manually operated flat roof windows, no impacts related to Furthermore, it includes the benefits of raw material substitution
maintenance are inventoried in module B2. Annual cleaning of the recycling of flat glass, with the exception of laminated
with water (e.g., using 1 l/m2 of tap water per annual cleaning) glass, which cannot be used for the production of glass again.
Recovered flat glass is assumed to have reached the end-of-
is neglected.
waste state as sorted glass cullet; glass cullet is assumed to
replace virgin raw material for glass production – impacts on
Module B6
the energy required to remelt recycled glass as compared to
Manually operated flat roof windows do not consume
virgin glass production are neglected due to a lack of data.
operational energy.
It also includes the benefits and loads related to the energy
Module C1
recovery from plastic wastes in a MWIP as modelled in
Manual de-installation is assumed, electricity consumption
Modules A3, A5 and C3.
related to electric screw drivers, etc. is considered to be
negligible. Thus, no environmental impacts are declared in
Due to a lack of data for plastics from de-construction activities,
module C1.
the substitution potential of recycled plastics is not taken into
account.
Module C2
Given the complexity of the inventoried products, a mixed end-
Only net flows leaving the product system are considered in
of-life scenario is modelled, allowing the different materials to
module D.
5 Environmental Product Declaration - VELUX A/S - VELUX flat roof window CXP
5. LCA: Results
Disclaimer:
EP-freshwater: This indicator has been calculated as 'kg P eq' as required in the characterization model (EUTREND model, Struijs et
al., 2009b, as implemented in ReCiPe; http://eplca.jrc.ec.europa.eu/LCDN/developerEF.xhtml)
DESCRIPTION OF THE SYSTEM BOUNDARY (X = INCLUDED IN LCA; MND = MODULE OR INDICATOR NOT DECLARED; MNR
= MODULE NOT RELEVANT)
Benefits and
Construction loads beyond
Product stage Use stage End of life stage
process stage the system
boundaries
la ire ta m w a Ry lp p u s tro p s n a rT g n iru tc a fu n a M e h t m o rf tro p s n a rTe tis e h t o t e ta g y lb m e s s A e s U e c n a n e tn ia M ria p e R tn e m e c a lp e R tn e m h s ib ru fe R y g re n e la n o ita re p Oe s u re ta w la n o ita re p Oe s u n o itc u rts n o c -e Dn o itilo m e d tro p s n a rT g n is s e c o rp e ts a W la s o p s iD -e s u e R-y re v o c e R-g n ilc y c e Rla itn e to p
A1 A2 A3 A4 A5 B1 B2 B3 B4 B5 B6 B7 C1 C2 C3 C4 D
X X X MND X X X MNR MNR MNR X MND X X X X X
RESULTS OF THE LCA - ENVIRONMENTAL IMPACT according to EN 15804+A2: 1 piece VELUX flat roof window CXP,
manually operated, 1.20 m x 1.20 m = 1.44 m2
Parameter Unit A1-A3 A5 B1 B2 B6 C1 C2 C3 C4 D
GWP-total kg CO 2 eq 2.6E+02 8.98E+00 0 0 0 0 7.02E-01 2.76E+00 9.64E+01 -5.9E+01
GWP-fossil kg CO 2 eq 2.68E+02 1.88E+00 0 0 0 0 7.02E-01 1.82E+00 9.63E+01 -5.89E+01
GWP-
biogenic kg CO 2 eq -8.03E+00 7.1E+00 0 0 0 0 0 9.36E-01 0 0
GWP-luluc kg CO 2 eq 2.57E-01 8.44E-05 0 0 0 0 2.86E-04 2.03E-03 3.26E-02 -1.01E-01
ODP kg CFC11 eq 5.78E-05 4.78E-08 0 0 0 0 1.65E-07 1.12E-07 1.11E-05 -3.65E-06
AP mol H+ eq 1.19E+00 1.31E-03 0 0 0 0 3.98E-03 6.96E-03 1.22E-01 -2.02E-01
EP-
kg P eq 8.19E-03 1.61E-06 0 0 0 0 5.16E-06 2.36E-04 9.65E-04 -3.93E-03
freshwater
EP-marine kg N eq 2.25E-01 4.91E-04 0 0 0 0 1.43E-03 2.23E-03 2.71E-02 -3.36E-02
EP-terrestrial mol N eq 2.42E+00 5.43E-03 0 0 0 0 1.57E-02 2.53E-02 2.99E-01 -3.83E-01
kg NMVOC
POCP 7.93E-01 1.53E-03 0 0 0 0 4.5E-03 6.75E-03 8.02E-02 -1.19E-01
eq
ADPE kg Sb eq 5.38E+02 6.99E-07 0 0 0 0 2.35E-06 3.17E-06 2.58E-04 3.73E-05
ADPF MJ 3.7E+03 3.13E+00 0 0 0 0 1.08E+01 2.52E+01 2.49E+02 -7.47E+02
m3 world eq
WDP 1.01E+02 1.27E-02 0 0 0 0 3.55E-02 6.26E-02 1.84E+01 -4.28E+00
deprived
GWP = Global warming potential; ODP = Depletion potential of the stratospheric ozone layer; AP = Acidification potential of land and water; EP =
Eutrophication potential; POCP = Formation potential of tropospheric ozone photochemical oxidants; ADPE = Abiotic depletion potential for non-fossil
resources; ADPF = Abiotic depletion potential for fossil resources; WDP = Water (user) deprivation potential)
RESULTS OF THE LCA - INDICATORS TO DESCRIBE RESOURCE USE according to EN 15804+A2: 1 piece VELUX flat roof
window CXP, manually operated, 1.20 m x 1.20 m = 1.44 m2
Parameter Unit A1-A3 A5 B1 B2 B6 C1 C2 C3 C4 D
PERE MJ 1.97E+02 4.74E-02 0 0 0 0 1.53E-01 3.18E+00 2.79E+01 -7.01E+01
PERM MJ 9.36E+01 -8.16E+01 0 0 0 0 0 -1.21E+01 0 0
PERT MJ 2.91E+02 -8.15E+01 0 0 0 0 1.53E-01 -8.88E+00 2.79E+01 -7.01E+01
PENRE MJ 3.45E+03 2.88E+01 0 0 0 0 1.08E+01 2.01E-05 1.15E+03 -7.54E+02
PENRM MJ 9.29E+02 -2.57E+01 0 0 0 0 0 0 -9.03E+02 0
PENRT MJ 4.38E+03 3.13E+00 0 0 0 0 1.08E+01 2.01E-05 2.49E+02 -7.54E+02
SM kg 2.25E+01 0 0 0 0 0 0 0 0 -6.77E+00
RSF MJ 0 0 0 0 0 0 0 0 0 0
NRSF MJ 0 0 0 0 0 0 0 0 0 0
FW m3 2.41E+00 6.25E-04 0 0 0 0 1.18E-03 6.01E-03 4.81E-01 -2.28E-01
PERE = Use of renewable primary energy excluding renewable primary energy resources used as raw materials; PERM = Use of renewable primary
energy resources used as raw materials; PERT = Total use of renewable primary energy resources; PENRE = Use of non-renewable primary energy
excluding non-renewable primary energy resources used as raw materials; PENRM = Use of non-renewable primary energy resources used as raw
materials; PENRT = Total use of non-renewable primary energy resources; SM = Use of secondary material; RSF = Use of renewable secondary fuels;
NRSF = Use of non-renewable secondary fuels; FW = Use of net fresh water
RESULTS OF THE LCA – WASTE CATEGORIES AND OUTPUT FLOWS according to EN 15804+A2:
1 piece VELUX flat roof window CXP, manually operated, 1.20 m x 1.20 m = 1.44 m2
Parameter Unit A1-A3 A5 B1 B2 B6 C1 C2 C3 C4 D
HWD kg 2.37E-02 8.25E-06 0 0 0 0 2.76E-05 2.01E-05 4.23E-04 1.84E-03
NHWD kg 5.83E+01 2.24E-01 0 0 0 0 7.24E-01 1.02E-01 3.79E+01 -9.41E+00
6 Environmental Product Declaration - VELUX A/S - VELUX flat roof window CXP
RWD kg 2.13E-02 4.45E-05 0 0 0 0 1.56E-04 2.28E-04 1.89E-03 -2.92E-03
CRU kg 0 0 0 0 0 0 0 0 0 0
MFR kg 1.05E+01 4.86E+00 0 0 0 0 0 1.57E+01 0 0
MER kg 0 0 0 0 0 0 0 0 0 0
EEE MJ 1.16E+00 3.34E+00 0 0 0 0 0 0 1.17E+02 0
EET MJ 2.2E+00 6.56E+00 0 0 0 0 0 0 2.31E+02 0
HWD = Hazardous waste disposed; NHWD = Non-hazardous waste disposed; RWD = Radioactive waste disposed; CRU = Components for re-use;
MFR = Materials for recycling; MER = Materials for energy recovery; EEE = Exported electrical energy; EET = Exported thermal energy
RESULTS OF THE LCA – additional impact categories according to EN 15804+A2-optional:
1 piece VELUX flat roof window CXP, manually operated, 1.20 m x 1.20 m = 1.44 m2
Parameter Unit A1-A3 A5 B1 B2 B6 C1 C2 C3 C4 D
Disease
PM 1.05E-05 1.93E-08 0 0 0 0 6.32E-08 1.08E-07 9.45E-07 -1.98E-06
incidence
IR kBq U235 eq 6.8E+00 1.35E-02 0 0 0 0 4.69E-02 8.73E-02 1.08E+00 -1.18E+00
ETP-fw CTUe 5.67E+03 3.27E+00 0 0 0 0 8.56E+00 1.48E+01 4.66E+03 -7.29E+02
HTP-c CTUh 4.94E-07 3.03E-10 0 0 0 0 3.41E-10 4E-10 3.01E-08 -3.39E-08
HTP-nc CTUh 4.7E-06 4.37E-09 0 0 0 0 9.85E-09 1.3E-08 1.17E-06 3.14E-08
SQP SQP 1.01E+03 2.63E+00 0 0 0 0 9.22E+00 3.4E+00 8.05E+01 -8.21E+01
PM = Potential incidence of disease due to PM emissions; IR = Potential Human exposure efficiency relative to U235; ETP-fw = Potential comparative
Toxic Unit for ecosystems; HTP-c = Potential comparative Toxic Unit for humans (cancerogenic); HTP-nc = Potential comparative Toxic Unit for humans
(not cancerogenic); SQP = Potential soil quality index
Disclaimer 1 – for the indicator 'Potential Human exposure efficiency relative to U235'.This impact category deals mainly with the
eventual impact of low dose ionizing radiation on human health of the nuclear fuel cycle. It does not consider effects due to possible
nuclear accidents, occupational exposure or radioactive waste disposal in underground facilities. Potential ionizing radiation from the
soil, radon and from some construction materials is also not measured by this indicator.
Disclaimer 2 – for the indicators 'abiotic depletion potential for non-fossil resources', 'abiotic depletion potential for fossil resources',
'water (user) deprivation potential, deprivation-weighted water consumption', 'potential comparative toxic unit for ecosystems', 'potential
comparative toxic unit for humans – cancerogenic', 'Potential comparative toxic unit for humans - not cancerogenic', 'potential soil
quality index'. The results of this environmental impact indicator shall be used with care as the uncertainties on these results are high
as there is limited experience with the indicator.
6. LCA: Interpretation
Figure 1 illustrates the relative contributions of the different
modules along the life cycle of the declared products.
Benefits and burdens beyond the system boundary (module D)
are in the order of 0 % to 40% of the impacts over the product
Figure1: Relative environmental impacts of the different life life cycle (modules A1-C4). [1] The use of renewable primary
cycle stages for the manually operated flat roof window energy is mainly caused by the share of renewable energy in
CXP the electricity mix, thus the production stage is the main driver
of this impact category; also for the use of non-renewable
The largest part of environmental impacts – between 70 % and primary energy, the production phase is the most impacting life
rather 100 % - is caused during production (modules A1-A3) of cycle stage.
the flat roof window. No operational energy is used as the flat Material use of primary energy is negligible and related to
roof window cannot be opened. plastic parts of the product and packaging material. The
7 Environmental Product Declaration - VELUX A/S - VELUX flat roof window CXP
material use of primary energy is transferred to its energy use wastes are mainly caused by the European electricity mix.
when the materials containing primary energy are incinerated
with energy recovery. [1] Benefits resulting from the recycling of plastics as well as
Non-hazardous waste as the quantitatively most relevant waste from the recycling of the electronic parts are disregarded due to
flows is mainly caused during the production of the glass and the lack of data on the recycling processes and related to the
during disposal of the product; hazardous and radio-active detailed composition of the electronic parts.
7. Requisite evidence
to AltholzVO
8.1 Formaldehyde Not applicable; not tested based on applicable product
Not tested based on applicable product standard. standard. 7.4. Fire gas toxicity
Not tested based on applicable product standard. 7.5 VOC
7.2 MDI emissions
Not tested based on applicable product standard. 7.3 Not tested based on applicable product standard.
Checking of pre-treatment of substances used according
8. References
Product category rules of IBU DIN EN 1873:2005, Prefabricated accessories for roofing -
Individual rooflights of plastics - Product specification and test
IBU (2021) methods.
IBU (2021): General Instructions for the EPD Programme of the
Institut Bauen & Umwelt e.V. (General Instructions for the IBU EN 16485
EPD Programme). Version 2.0, Institut Bauen & Umwelt, Berlin DIN EN 16485:2014-07, Round and sawn timber -
Environmental Product Declarations - Product category rules
IBU (2017) for wood and wood-based products for use in construction;
IBU (2017): PCR Teil A: PCR Part A: Calculation rules for the German version EN 16485:2014.
life cycle assessment and requirements for the project report.
Version 1.8., Institut Bauen & Umwelt, Berlin. ECHA-List
The Candidate List of substances of very high concern,
IBU (2021) available via https://echa.europa.eu/nl/-/four-newsubstances-
IBU (2021):PCR Part B: Requirements on the EPD for windows added-to-the-candidate-list.
and doors. Version 2021/01, Institut Bauen & Umwelt, Berlin.
Regulation on biocidal products
Standards and legal documents REGULATION (EU) No 528/2012 OF THE EUROPEAN
PARLIAMENT AND OF THE COUNCIL of 22 May 2012
EN 15804 concerning the making available on the market and use of
DIN EN 15804+A2:2019, Sustainability of construction works - biocidal products.
Environmental product declarations - Core rules for the product
category construction products. Regulation (EU) Nr. 305/2011(CPR)
REGULATION (EU) No 305/2011 OF THE EUROPEAN
ISO 14025 PARLIAMENT AND OF THE COUNCIL of 9 March 2011 laying
DIN EN ISO 14025:2006-07, Environmental labels and down harmonised conditions for the marketing of construction
declarations - Type III Environmental declarations - Principles products and repealing Council Directive 89/106/EEC.
and procedures.
COUNCIL REGULATION (EU) No 333/2011
ISO 14044 COUNCIL REGULATION (EU) No 333/2011 of 31 March 2011
DIN EN ISO 14044:2006-07, Environmental management - Life establishing criteria determining when certain types of scrap
cycle assessment - Requirements and guidance (ISO metal cease to be waste under Directive 2008/98/EC of the
14044:2006); German and English versions EN ISO European Parliament and of the Council.
14044:2006.
European Waste List (Waste index)
ISO 9001 http://www.gesetze-im-internet.de/avv/anlage.htm
DIN EN ISO 9001:2015, Quality management systems -
Requirements. Additional references
ISO 14001 Weidema et al. (2013)
DIN EN ISO 14001:2015: Environmental management Weidema, B., C. Bauer, R. Hischier, C. Mutel, T. Nemecek, J.
systems - Requirements with guidance for use. Reinhard, C.O. Vadenbo, G. Wernet (2013): Overview and
methodology, Data quality guideline for the ecoinvent database
ISO 45001 version 3. ecoinvent report no. 1 (v3), St. Gallen, Schweiz.
ISO 45001:2018-03, Occupational health and safety
management systems - Requirements with guidance for use. ecoinvent 3.8
ecoinvent 3.8, LCA database, 12/2021. Ecoinvent centre,
EN 1873 Zürich.
8 Environmental Product Declaration - VELUX A/S - VELUX flat roof window CXP
Publisher
Institut Bauen und Umwelt e.V. +49 (0)30 3087748- 0
Hegelplatz 1 info@ibu-epd.com
10117 Berlin www.ibu-epd.com
Germany
Programme holder
Institut Bauen und Umwelt e.V. +49 (0)30 3087748- 0
Hegelplatz 1 info@ibu-epd.com
10117 Berlin www.ibu-epd.com
Germany
Author of the Life Cycle Assessment
Dr. Frank Werner - Umwelt & Entwicklung + 41 (0)44 241 39 06
Kammelenbergstrasse 30 frank@frankwerner.ch
9011 St. Gallen http://www.frankwerner.ch/
Switzerland
Owner of the Declaration
VELUX Group +4545164726
Ådalsvej 99 jakob.roerbech@velux.com
2970 Hørsholm www.velux.com
Denmark
9 Environmental Product Declaration - VELUX A/S - VELUX flat roof window CXP
