ENVIRONMENTAL PRODUCT DECLARATION
as per ISO 14025 and EN 15804+A2
Owner of the Declaration HILTI AG
Programme holder Institut Bauen und Umwelt e.V. (IBU)
Publisher Institut Bauen und Umwelt e.V. (IBU)
Declaration number EPD­HIL­20220211­ICA1­EN
Issue date 21.09.2022
Valid to 20.09.2027
Hilti CFS­F­FX
HILTI AG
www.ibu-epd.com | https://epd-online.com
Umwelt Produktdeklaration Name des Herstellers – Name des Produkts
1. General Information
HILTI Hilti CFS­F­FX
Programme holder Owner of the declaration
IBU – Institut Bauen und Umwelt e.V. Hilti AG
Hegelplatz 1 Feldkircher Str. 100
10117 Berlin FL­9494 Schaan
Germany Liechtenstein
Declaration number Declared product / declared unit
EPD­HIL­20220211­ICA1­EN The declared product is a HILTI firestop foam CFS­F­
FX. The declared unit is one kilogram of reaction resin
product in the mixing ratio of the two components
necessary for processing. The packaging is also
included in the calculation. The declared unit is stated
in [kg].
This declaration is based on the product Scope:
category rules: This document refers to the CFS­F­FX firestop foam
Reaction resin products, 01.2019 with its packaging. Specific data from 2021 were
(PCR checked and approved by the SVR) collected from Hilti's manufacturing plant in Kaufering,
Germany and used for this environmental Life Cycle
Assessment.
Issue date
21.09.2022
The owner of the declaration shall be liable for the
underlying information and evidence; the IBU shall not
Valid to
be liable with respect to manufacturer information, life
20.09.2027
cycle assessment data and evidences.
The EPD was created according to the specifications
of EN 15804+A2. In the following, the standard will be
simplified as EN 15804.
The owner of the declaration shall be liable for the
underlying information and evidence; the IBU shall not
be liable with respect to manufacturer information, life
cycle assessment data and evidences.
The EPD was created according to the specifications
of EN 15804+A2. In the following, the standard will be
simplified as EN 15804.
Verification
The standard EN 15804 serves as the core PCR
Independent verification of the declaration and data
according to ISO 14025:2011
Dipl. Ing. Hans Peters internally x externally
(chairman of Institut Bauen und Umwelt e.V.)
Dr. Alexander Röder Matthias Klingler
(Managing Director Institut Bauen und Umwelt e.V.)) (Independent verifier)
2. Product
2.1 Product description/Product definition following purposes: waste volume reduction, easy
storage and transport, and less packaging material.
Through legislation and increased public awareness
The declared product of CFS­F FX is a two­component users have increasingly become discerned towards the
system. These are: a polyol based Component A and a use of styrene and other highly volatile components
diisocyanate based Component B. Mixing the 2 with their resulting unpleasant odour and low flash
components A and B in the static mixer initiates the point (flammability).
curing (hardening) reaction of both systems to form a The reaction resins used in the product contain no
cured Polyurethane Foam in the application. styrene, are practically odourless and have a
Composite foils are used for the two­component foil considerably higher flash point, i.e. higher than 100 °C
pack of CFS­F FX. This kind of packaging serves the in comparison to 34 °C for styrene­based products.
2 Environmental Product Declaration Hilti – Hilti CFS­F FX
CFS­F FX is the ultimate easy­to­install flexible firestop Other: 5­15 %
foam to help create a fire and smoke barrier around
cable and mixed penetrations. This product article contains substances listed in the
For the placing of the product on the market in the candidate list (date: 07.04.2022) exceeding 0.1
European Union European Free Trade Association percentage by mass: no.
EU/EFTA) (with the exception of Switzerland)
Regulation (EU) No. 305/2011 (CPR) applies. The This product contains other carcinogenic, mutagenic,
product needs a declaration of performance taking into reprotoxic (CMR) substances in categories 1A or 1B
consideration the following European Technical which are not on the candidate list, exceeding 0.1
Approval: ETA-10/0109 and the CE­marking. For the percentage by mass: no.
application and use the respective national provisions
apply. Biocide products were added to this construction
product or it has been treated with biocide products
2.2 Application (this then concerns a treated product as defined by the
Hilti CFS­F FX serves to form a penetration seal, which (EU) Ordinance on Biocide Products No. 528/2012):
is used to maintain the fire resistance of a concrete, no.
masonry or drywall separating element (wall or floor)
when and where services (cables, metal or plastic
pipes, etc.) pass through. 2.6 Manufacture
Most raw materials are sourced in Europe. The
2.3 Technical Data transport is exclusively by truck for the European raw
materials, and by truck and by ship for the others.
The production of the chemical firestop foam consists
Constructional data of a mixing process and a filling process of the
Name Value Unit respective single components (A and B) and their
Density EN ISO 1183­1 1260 kg/m3 subsequent combination in a two­component system
(packaging). Here process control technology is used
to weigh and mix solid and liquid compounds
according to the specification. In the next step both
Hilti CFS-F FX displays the following well­mixed components run through an automized
characteristics: filling line in which each of the processed masses is
filled into a tubular foil bag. Finally, the single
Performance data of the product in accordance with components are combined in one packaging unit. The
the declaration of performance with respect to its two­pack foil bags are packed into cardboard boxes
essential characteristics according to and then finally shipped. The manufacturing plant of
ETA-10/0109 CFS­F FX, Hilti GmbH Industriegesellschaft für
Befestigungstechnik, Hiltistr. 6, 86916 Kaufering,
Shelf life of 9 months: Germany, is certified according to ISO 9001. The
Substrate temperature during installation 0 to +40 °C guideline defines international standards for quality
(internal method). and process management.
The following flowcharts illustrate the underlying
Curing time: approx. 10 min production process
2.4 Delivery status
The product Hilti CFS­F­FX is available in foil­
packages with 325 ml injectable foam in the
corresponding mixing ratio. 1 package of CFS­F FX
contains 0.41 kg of reaction resin.
2.5 Base materials/Ancillary materials
Hilti CFS­F FX is supplied in the form of a dual
component film­wrapped pack comprising a
component A and component B at a weight ratio of 3:1.
The mixing ratio of resin and curing agent components
is automatically set during the injection process.
Product curing commences directly after the
components are mixed. Illustration: Production process of the reaction
resin mixture
The product reviewed in this EPD contains the
following component volumes:
Component A:
Polyol: 30­40 %
Intumescent Flame Retardant: 15­25 %
Polymer dispersion: 25­35 %
Fungicide: ≤ 5 %
Manufacturing agent: ≤ 5 %
Other: ≤ 5 %
Component B:
Diisocyanate: 85­95 %
3 Environmental Product Declaration Hilti – Hilti CFS­F FX
Hilti literature and official approvals must always be
considered. The two components of CFS­F FX are
only for use in combination with the defined volume
ratio and under the conditions mentioned above.
2.11 Environment and health during use
Refer to the Safety Data Sheet (SDS) for detailed
information on handling, storage as well as first aid,
firefighting and accidental release measures and
disposal considerations. Following the given
instructions helps to minimize the risk to health and the
Illustration: Production process of the packaging environment.
2.7 Environment and health during 2.12 Reference service life
manufacturing Hilti CFS­F FX is exposed to a wide variety of
The manufacturing plant of CFS­F FX,Hilti GmbH environmental factors during the use phase. The
Industriegesellschaft für Befestigungstechnik, Hiltistr. anticipated Reference Service Life depends on the
6, 86916 Kaufering, Germany, is certified according to specific installation situation and the product exposure
ISO 14001 which defines international standards for scenarios. The main factors influencing the period of
sustainable environmental management. The use involve weathering as well as mechanical loads
production site is also certified in accordance with DIN and chemical exposure.
EN ISO 50001 Energy Management Systems.
2.8 Product processing/Installation 2.13 Extraordinary effects
The product is delivered with Instructions for Use
explaining the basic steps for installation: Fire
The CFS­F FX (at cured state) complies with the
1) For safe handling the precautionary measures requirements of the DIN EN 13501-1 standard for fire
described in the Safety Data Sheet (SDS) (e.g. hand classes E and Efl. The product’s resistance to fire is
and eye protection) must be adhered to detailed in Annex 2 of ETA 10/0109 approval
2) Insert the cartridge into the black cassette document.
3) Screw on the mixing nozzle
4) Put the cassette into the dispenser system Fire protection
5) Inject the foam in the opening to be sealed Name Value
6) If necessary, shape the foam by hand Building material class E/Efl
No performence
Burning droplets
After the curing time, described in Instructions for Use, assessed
the application is complete. Foam excesses can be cut No performence
Smoke gas development
and placed in further openings to be sealed. assessed
2.9 Packaging Water
Hilti CFS­F FX is supplied in the form of a 2­foil­pack The cured product is chemically inert and insoluble in
system and thus leads to very little waste remaining water.
after use on the construction site. After curing, the
product can be disposed of with household waste. Full Mechanical destruction
or only partially emptied cartridges must be disposed It is recommended to use dust protection during the
of as special waste in accordance with official demolition of the cured foam.
regulations.
The outer packaging consisting of plastic / aluminium 2.14 Re-use phase
foil and cardboard boxes designed according to the The product cannot be re­used. After usage the
product size can be recycled. Packaging contaminated product can be removed by demolition.
by the product must be disposed in a safe manner in
accordance with local/national regulations. 2.15 Disposal
Uncured Hilti CFS­F­FX can be disposed of according
to the European waste code 08 04 09* or 20 01 27*.
2.10 Condition of use
During the installation the temperature of the base 2.16 Further information
material must be between 0° C and +40° C. The Further information is available on the Hilti website:
temperature of the product should be between 5 and www.hilti.group
25° C during storage and 10 and 35° C during usage.
3. LCA: Calculation rules
3.1 Declared Unit product is also included in the calculation. 1 package
The declared product is a HILTI firestop foam CFS­F of CFS­F FX contains 0.41kg of reaction resin. The
FX. The declared unit refers to one kilogram of following table shows the data of the declared unit.
reaction resin product in the required mixing ratio of
the two components. The packaging of 0,267 kg/kg of Declared unit
4 Environmental Product Declaration Hilti – Hilti CFS­F FX
Name Value Unit production processes. In some cases, assumptions
Declared unit 1 kg were made because of a lack of primary or secondary
data, in particular for the following aspects:
 The synthesis way of raw materials which
were not available on the Ecoinvent database
3.2 System boundary
was used to reconstruct these material's
The type of EPD is cradle to grave. The following
impact
information modules are defined as system boundaries
 Some raw material's packaging composition
in this study:
and transportation distances were estimated
A1 – Raw material supply:  Estimations were made to calculate the
Production and packaging of the raw materials to be energy consumption during installation
supplied to the manufacturer. All processes are
 The transportation scenario to the building
included from cradle to gate.
site is based on french transportation
A2 – Transport (to manufacturing site):
companies' statistics.
Transportation of all the raw materials and their
packaging between their production site and the
manufacturing site, for all transport modes (sea, road).
A3 – Manufacturing: 3.4 Cut-off criteria
Production, supply and use of energy sources at the All information modules considered were included in
manufacturing sites (electricity, biomass and natural the calculation in such detail that all requirements of
gas). Green electricity from wind turbines is EN 15804 are met. The consumption of additional
considered for the whole manufacturing process. inputs such as lubricants, oils or solvents used for
Production and transport of production losses, final manufacture is less than 5 % by weight and therefore
product packaging and other inputs. falls below the cut­off criterion of the total calculation.
End­of­life of production waste (hazardous, non­
hazardous and recyclable), production losses and raw 3.5 Background data
material packaging, including waste and losses The source for background data for the LCA
transportation, processing and disposal. calculations is the ecoinvent 3.8 database.
A4 – Transport (to construction site)
Transportation of packaged products from the 3.6 Data quality
manufacturing site to the construction site, including For the compilation of the life cycle assessment,
potential in­betweens (retailer, workshop, etc.). specific data were collected from the factory Kaufering,
A5 – Installation­Construction in Germany, of the HILTI AG from the year 2018. The
Electricity consumption for injecting (in case of background data from the ecoinvent 3.8 database
injection with electrical dispenser). used was updated in the year 2021. The mass of the
Production of the construction losses. different components of the reactive resin mixture
Provision and end­of­life of tools and accessories for come from the information in the recipe. The data
injectable mortars (manual or electrical dispenser with quality is classified as appropriate.
or without battery and with cartridge holder).
End­of­life of hazardous construction losses and 3.7 Period under review
packaging (uncured resin and soiled packaging) and Data from the year 2021 are used, which correspond
non­hazardous construction losses (cured foam and to the annual average.
unsoiled packaging): including waste transportation,
processing and disposal. 3.8 Allocation
C1 – Deconstruction/demolition The used operating tools (stage A5), which are Hilti's
Diesel for building demolition. manual or electrical dispenser can be used to inject the
C2 – Transport (to waste processing) CFS­F FX as well as other Hilti products. The part of
Transportation to waste processing facility. the dispenser's impact allocated to the current product
C4– Waste disposal is based on the estimated total mass of injected
Treatment and disposal of plastic to sanitary landfill. product each dispenser can be used for. This can be
considered a mass allocation.
For the environmental impact, the use of green
electricity (stage A3) was calculated taking into 3.9 Comparability
account the residual electricity mix for the remaining Basically, a comparison or an evaluation of EPD data
electricity. The proportion of the electricity demand is only possible if all the data sets to be compared
covered by green electricity in the total electricity were created according to EN 15804 and the building
demand is 100%. context, respectively the product­specific
characteristics of performance, are taken into account.
3.3 Estimates and assumptions The used background database is given by ecoinvent
3.8 database, to which this study refers.
In general, background data and electricity mixes are
chosen and calculated country­specifically for the
4. LCA: Scenarios and additional technical information
Characteristic product properties Information on biogenic Carbon
The declared product contains 90 g of paper and
cardboard (outer packaging and user manual). Since
5 Environmental Product Declaration Hilti – Hilti CFS­F FX
only these materials contain biogenic carbon, in
addition to a neglectable part contained in the raw
materials' packaging, all the biogenic carbon capture
and release were cancelled to simplify the model.
The cancelled emission corresponds to 0,012 kg of
biogenic carbon (0,0438 kg of CO ) for a cancelled
2
capture of 0,022 kg of biogenic carbon (0,0818 kg of
CO ).
2
The following scenarios were considered for the LCA
calculations:
Transport to the building site (A4)
Name Value Unit
Transport distance 900 km
lorry 16­32
Vehicle type ­
metric ton
Effective load 21 t
Maximum capacity 24 t
Consumption when unloaded 0,25 L/km
Consumption at full capacity 0,38 L/km
Empty return rate 14 %
Effective consumption 0,019 L/tkm
Installation into the building (A5)
Name Value Unit
Water consumption ­ m3
Electricity consumption 0.0004 kWh
Uncured foam loss 0.04 kg
Cured foam loss 0.00 kg
Total foam loss 0.04 kg
Hazardous waste (soiled
0.177 kg
packaging)
Non­hazardous waste for
0.090 kg
recycling (unsoiled packaging)
End of life (C1-C4)
Name Value Unit
Fuel for building demolition 0,0437 MJ
Distance to sanitary landfill 50 km
Landfilling 1 kg
6 Environmental Product Declaration Hilti – Hilti CFS­F FX
5. LCA: Results
DESCRIPTION OF THE SYSTEM BOUNDARY (X = INCLUDED IN LCA; ND = MODULE OR INDICATOR NOT
DECLARED; MNR = MODULE NOT RELEVANT)
BENEFITS AND
CONSTRUCTI LOADS
PRODUCT STAGE ON PROCESS USE STAGE END OF LIFE STAGE BEYOND THE
STAGE SYSTEM
BOUNDARIES
7 Environmental Product Declaration Hilti – Hilti CFS­F FX
lairetam
waR
ylppus tropsnarT
gnirutcafunaM
eht
morf
tropsnarT
etis
eht
ot
etag
ylbmessA esU
ecnanetniaM
riapeR
tnemecalpeR tnemhsibrufeR
ygrene
lanoitarepO esu
retaw
lanoitarepO esu
noitcurtsnoc­eD
noitilomed tropsnarT
gnissecorp
etsaW
lasopsiD ­esueR ­yrevoceR ­gnilcyceR laitnetop
A1 A2 A3 A4 A5 B1 B2 B3 B4 B5 B6 B7 C1 C2 C3 C4 D
X X X X X ND ND MNR MNR MNR ND ND X X X X X
RESULTS OF THE LCA - ENVIRONMENTAL IMPACT according to EN 15804+A2: 1 kg CFS-F-FX
Core Indicator Unit A1 A2 A3 A4 A5 C1 C2 C3 C4 D
GWP­total [kg CO2­Eq.] 3.35E+0 4.03E­2 8.87E­1 7.89E­2 7.56E­1 4.02E­3 4.84E­3 0.00E+0 1.14E­1 0.00E+0
GWP­fossil [kg CO2­Eq.] 3.26E+0 4.01E­2 8.72E­1 7.86E­2 7.50E­1 4.02E­3 4.82E­3 0.00E+0 1.14E­1 0.00E+0
GWP­biogenic [kg CO2­Eq.] 8.23E­2 1.08E­4 1.35E­2 2.73E­4 5.84E­3 3.65E­6 1.67E­5 0.00E+0 2.85E­4 0.00E+0
GWP­luluc [kg CO2­Eq.] 3.01E­3 2.10E­5 1.24E­3 3.14E­5 3.32E­4 4.00E­7 1.93E­6 0.00E+0 2.15E­6 0.00E+0
ODP [kg CFC11­Eq.] 2.63E­5 8.95E­9 3.13E­7 1.82E­8 1.13E­6 8.59E­10 1.12E­9 0.00E+0 3.10E­9 0.00E+0
AP [mol H+­Eq.] 2.64E­2 3.74E­4 4.57E­3 2.23E­4 2.69E­3 4.17E­5 1.37E­5 0.00E+0 7.63E­5 0.00E+0
EP­freshwater [kg P­Eq.] 1.55E­3 2.45E­6 2.80E­4 5.38E­6 2.43E­4 1.27E­7 3.30E­7 0.00E+0 8.58E­7 0.00E+0
EP­marine [kg N­Eq.] 4.74E­3 8.24E­5 9.27E­4 4.56E­5 4.61E­4 1.85E­5 2.79E­6 0.00E+0 2.14E­3 0.00E+0
EP­terrestrial [mol N­Eq.] 3.48E­2 9.13E­4 8.39E­3 4.95E­4 5.84E­3 2.03E­4 3.03E­5 0.00E+0 3.07E­4 0.00E+0
POCP [kg NMVOC­Eq.] 1.29E­2 2.64E­4 2.79E­3 1.90E­4 1.25E­3 5.57E­5 1.17E­5 0.00E+0 1.12E­4 0.00E+0
ADPE [kg Sb­Eq.] 7.55E­5 1.26E­7 4.51E­6 2.84E­7 8.69E­6 2.04E­9 1.74E­8 0.00E+0 3.11E­8 0.00E+0
ADPF [MJ] 6.74E+1 5.74E­1 1.93E+1 1.17E+0 6.57E+0 5.41E­2 7.17E­2 0.00E+0 2.22E­1 0.00E+0
[m³ world­Eq
WDP 2.52E+0 2.53E­3 3.67E­1 5.48E­3 2.13E­1 1.45E­4 3.36E­4 0.00E+0 2.30E­3 0.00E+0
deprived]
GWP = Global warming potential; ODP = Depletion potential of the stratospheric ozone layer; AP = Acidification potential of land and water; EP =
Caption Eutrophication potential; POCP = Formation potential of tropospheric ozone photochemical oxidants; ADPE = Abiotic depletion potential for non­
fossil resources; ADPF = Abiotic depletion potential for fossil resources; WDP = Water (user) deprivation potential
RESULTS OF THE LCA - INDICATORS TO DESCRIBE RESOURCE USE according to EN 15804+A2: 1 kg
CFS-F-FX
Indicator Unit A1 A2 A3 A4 A5 C1 C2 C3 C4 D
PERE [MJ] 4.14E+0 7.53E­3 1.08E+0 1.70E­2 3.45E­1 3.09E­4 1.04E­3 0.00E+0 1.17E­2 0.00E+0
PERM [MJ] 1.32E­2 0.00E+0 7.33E­1 0.00E+0 2.98E­2 0.00E+0 0.00E+0 0.00E+0 0.00E+0 0.00E+0
PERT [MJ] 4.16E+0 7.53E­3 1.81E+0 1.70E­2 3.74E­1 3.09E­4 1.04E­3 0.00E+0 1.17E­2 0.00E+0
PENRE [MJ] 4.73E+1 5.74E­1 1.39E+1 1.17E+0 5.51E+0 5.41E­2 7.17E­2 0.00E+0 2.22E­1 0.00E+0
PENRM [MJ] 2.46E+1 0.00E+0 5.46E+0 0.00E+0 1.24E+0 0.00E+0 0.00E+0 0.00E+0 0.00E+0 0.00E+0
PENRT [MJ] 7.19E+1 5.74E­1 1.94E+1 1.17E+0 6.75E+0 5.41E­2 7.17E­2 0.00E+0 2.22E­1 0.00E+0
SM [kg] 2.52E­2 2.22E­4 9.04E­2 3.98E­4 6.62E­3 2.12E­5 2.44E­5 0.00E+0 8.41E­5 0.00E+0
RSF [MJ] 4.93E­4 1.86E­6 8.42E­3 4.38E­6 3.90E­4 6.91E­8 2.69E­7 0.00E+0 3.83E­6 0.00E+0
NRSF [MJ] 0.00E+0 0.00E+0 0.00E+0 0.00E+0 0.00E+0 0.00E+0 0.00E+0 0.00E+0 0.00E+0 0.00E+0
FW [m³] 7.13E­2 6.64E­5 1.01E­2 1.49E­4 5.59E­3 3.28E­6 9.14E­6 0.00E+0 2.92E­4 0.00E+0
PERE = Use of renewable primary energy excluding renewable primary energy resources used as raw materials; PERM = Use of
renewable primary energy resources used as raw materials; PERT = Total use of renewable primary energy resources; PENRE = Use of
non­renewable primary energy excluding non­renewable primary energy resources used as raw materials; PENRM = Use of non­
Caption
renewable primary energy resources used as raw materials; PENRT = Total use of non­renewable primary energy resources; SM = Use
of secondary material; RSF = Use of renewable secondary fuels; NRSF = Use of non­renewable secondary fuels; FW = Use of net fresh
water
RESULTS OF THE LCA – WASTE CATEGORIES AND OUTPUT FLOWS according to EN 15804+A2:
1 kg CFS-F-FX
Indicator Unit A1 A2 A3 A4 A5 C1 C2 C3 C4 D
HWD [kg] 5.59E­1 7.10E­4 6.17E­2 1.33E­3 3.46E­1 7.23E­5 8.16E­5 0.00E+0 3.46E­4 0.00E+0
NHWD [kg] 6.84E+0 1.07E­2 1.43E+0 2.37E­2 5.40E­1 5.08E­4 1.45E­3 0.00E+0 1.00E+0 0.00E+0
RWD [kg] 1.54E­4 3.97E­6 3.20E­5 8.05E­6 2.51E­5 3.81E­7 4.93E­7 0.00E+0 1.47E­6 0.00E+0
CRU [kg] 0.00E+0 0.00E+0 0.00E+0 0.00E+0 0.00E+0 0.00E+0 0.00E+0 0.00E+0 0.00E+0 0.00E+0
MFR [kg] 4.69E­4 1.88E­5 3.59E­2 3.67E­6 9.51E­2 7.20E­8 2.25E­7 0.00E+0 1.21E­6 0.00E+0
MER [kg] 7.17E­6 1.48E­8 5.93E­7 2.95E­8 4.94E­7 1.15E­9 1.81E­9 0.00E+0 5.85E­9 0.00E+0
EEE [MJ] 4.07E­2 1.15E­4 1.08E­2 2.55E­4 3.58E­3 2.12E­5 1.56E­5 0.00E+0 4.53E­4 0.00E+0
EET [MJ] 1.42E­1 5.68E­4 3.40E­2 1.06E­3 1.21E­2 2.15E­4 6.49E­5 0.00E+0 1.22E­3 0.00E+0
HWD = Hazardous waste disposed; NHWD = Non­hazardous waste disposed; RWD = Radioactive waste disposed; CRU = Components
Caption for re­use; MFR = Materials for recycling; MER = Materials for energy recovery; EEE = Exported electrical energy; EET = Exported
thermal energy
RESULTS OF THE LCA – additional impact categories according to EN 15804+A2-optional:
1 kg CFS-F-FX
Indicator Unit A1 A2 A3 A4 A5 C1 C2 C3 C4 D
[Disease
PM 1.96E­7 2.74E­9 4.66E­8 6.34E­9 2.44E­8 1.12E­9 3.88E­10 0.00E+0 1.62E­9 0.00E+0
Incidence]
[kBq U235­
IRP 4.19E­1 2.93E­3 7.83E­2 6.14E­3 4.06E­2 2.48E­4 3.76E­4 0.00E+0 1.48E­3 0.00E+0
Eq.]
ETP­fw [CTUe] 2.35E+2 4.57E­1 1.55E+1 9.76E­1 2.40E+1 3.25E­2 5.98E­2 0.00E+0 4.83E­1 0.00E+0
HTP­c [CTUh] 2.87E­8 1.85E­11 6.67E­10 3.00E­11 1.58E­9 1.25E­12 1.84E­12 0.00E+0 7.12E­12 0.00E+0
HTP­nc [CTUh] 2.84E­7 4.21E­10 1.18E­8 9.56E­10 1.69E­8 2.35E­11 5.86E­11 0.00E+0 1.81E­10 0.00E+0
SQP [­] 1.22E+1 3.37E­1 6.87E+0 8.31E­1 1.57E+0 7.03E­3 5.09E­2 0.00E+0 5.83E­1 0.00E+0
PM = Potential incidence of disease due to PM emissions; IR = Potential Human exposure efficiency relative to U235; ETP­fw = Potential
Caption comparative Toxic Unit for ecosystems; HTP­c = Potential comparative Toxic Unit for humans (cancerogenic); HTP­nc = Potential
comparative Toxic Unit for humans (not cancerogenic); SQP = Potential soil quality index
Disclaimer 1 – for the indicator “Potential Human exposure efficiency relative to U235”.This impact category
deals mainly with the eventual impact of low dose ionizingradiation on human health of the nuclear fuel cycle. It
does not consider effects due to possiblenuclear accidents, occupational exposure or radioactive waste disposal
in undergroundfacilities. Potential ionizing radiation from the soil, radon and from some construction materials is
also not measured by this indicator.
Disclaimer 2 – for the indicators “abiotic depletion potential for non­fossil resources”, “abiotic depletion potential
for fossil resources”, “water (user) deprivation potential, deprivation­weighted water consumption”, “potential
comparative toxic unit for ecosystems”, “potential comparative toxic unit for humans – cancerogenic”, “Potential
comparative toxic unit for humans ­ not cancerogenic”, “potential soil quality index”. The results of this
environmental impact indicator shall be used with care as theuncertainties on these results are high as there is
limited experience with the indicator.
6. LCA: Interpretation
The dominance analysis shows that the main causes In the information module A1, the material supply of
of environmental impacts and indicators can be found the reaction resin mixture causes more than 90 % of
in information module A1. This shows the global the global warming potential.
warming potential for the provision of material with
more than 50 %, based on all information modules.
Modules A3 and A5 also represent important parts of
the final impact.
Illustration: Dominance analysis A1
The mass of the individual components of the reaction
resin mixture come from the recipe information
provided by the manufacturer. According to the
manufacturer, this information can be assumed to be
Illustration: Dominance analysis A1- C4
highly accurate.
The relevant datasets used to calculate the material
Module A1 is detailed below. Module A3’s global
availability of the product are highly topical since the
warming impact is mostly constituted by the final
raw materials were detailed as much as necessary to
product packaging (13 % of the total impact) but also
find corresponding data in the latest Ecoinvent
the energy consumption (2 % of the final impact). Most
database (2021). The locations were also respected.
of the global warming impact from module A5 is
Since these datasets strongly influence the results, as
caused by the product losses (3 % of the final impact)
shown by the dominance analysis, so does the overall
the end­of­life of the soiled product packaging, and
computation.
treated as hazardous waste (9 % of the final impact).
7. Requisite evidence
with the eco­Institute test report no. 55493­
Hilti CFS­F­FX complies with the requirements of C006
 AgBB­Scheme for the health evaluation of
construction products (2018), in accordance
8 Environmental Product Declaration Hilti – Hilti CFS­F FX
 Emission class A+ according to the French
VOC Labelling regulation and CMR emissions
regulation in accordance with the eco­Institute
AgBB overview of results (28 days [µg/m³])
test report no. 55493­C006 III
Name Value Unit
 Belgian Royal Decree establishing threshold TVOC (C6 ­ C16) 46 μg/m3
levels for the emissions to the indoor Sum SVOC (C16 ­ C22) 0 ­ 5 μg/m3
environment from construction products for R (dimensionless) 0.08 ­
specific purposes in accordance with the eco­ VOC without NIK 26 μg/m3
Institute test report no. 55493­C006 II Carcinogenic Substances 0 ­ 1 μg/m3
 CDPH Standard Method V1.2­2017 according
AgBB overview of results (3 days [µg/m³])
to the eco­institut test report no. B55493­
Name Value Unit
B006) from 11.11.2020.
TVOC (C6 ­ C16) 120 μg/m3
Carcinogenic Substances 0 ­ 1 μg/m3
8. References
Standards PCR Part A
Institut Bauen und Umwelt e.V, Berlin (pub.):
EN 13501-1 Product Category Rules for Construction Products
DIN EN 13501­1 : 2018 Fire classification of from the range of Environmental Product Declarations
construction products and building elements. for Institut Bauen und Umwelt (IBU), Part A:
Calculation Rules for the Life Cycle Assessment and
EN 14293 Requirements on the Project Report according to EN
DIN EN 14293 : 2006 Adhesives ­ Adhesives for 15804+A2:2019, 2021­04
bonding parquet to subfloor ­ Test methods and
minimum requirements PCR Part B
Institut Bauen und Umwelt e.V, Berlin (pub.):
EN 15804 Product Category Rules for Construction Products
EN 15804:2012+A2:2019, Sustainability of from the range of Environmental Product Declarations
construction works — Environmental Product for Institut Bauen und Umwelt (IBU), Part B:
Declarations — Core rules for the product category of Requirements on the EPD for Reaction resin products,
construction products. 2019­01
EN ISO 604
DIN EN ISO 604:2003­12: Determination of
compressive properties Further References
EN ISO 1183-1 AFNOR, «FD P01-015» 2006
DIN 51757:2011­01 Plastics ­ Methods for determining Qualité environnementale des produits de construction
the density of non­cellular plastics ­ Part 1: Immersion ­ Fascicule de données énergie et transport
method, liquid pyknometer method and titration
method AgBB (2018)
Vorgehensweise bei der gesundheitlichen
EN ISO 50001 Bewertung der Emissionen von flüchtigen
DIN EN ISO 50001: 2018 Energy management organischen Verbindungen (VVOC, VOC und SVOC)
systems ­ Requirements with guidance for use aus Bauprodukten (2018)
IBU 2021 Candidate List of substances of very high concern
Institut Bauen und Umwelt e.V.: General Instructions for Authorisation
for the EPD programme of Institut Bauen und Umwelt European Cheminals Agency (ECHA), in accordance
e.V., Version 2.0, Berlin: Institut Bauen und Umwelt with Article 50(10) of the REACH regulation
e.V., 2021
www.ibu­epd.com CDPH/EHLB/Standard Method V1.2
California CDPH Standard Method is a US standard
ISO 9001 for evaluating and restricting VOC emissions to indoor
ISO 9001:2015 Quality management systems ­ air. Developed in California as "Section
Requirements 01350" Specification, several systems in the US refer
to CDPH Standard Method
ISO 14001
ISO 14001:2015 Environmental management systems Comité National Routier (CNR)
­ Requirements with guidance for use Enquête longue distance, PARIS, 2019
ISO 14025 CPR
EN ISO 14025:2011, Environmental labels and Regulation (EU) No 305/2011 of the European
declarations — Type III environmental declarations — Parliament and of the Council of 9 March 2011 laying
Principles and procedures. down harmonised conditions for the marketing of
9 Environmental Product Declaration Hilti – Hilti CFS­F FX
construction products and repealing Council Directive
89/106/EEC NSF
NSF/ANSI/CAN 61 Drinking Water System
DIBt (2010) Components ­ Health Effects
Grundsätze zur gesundheitlichen Bewertung
von Bauprodukten in Innenräumen (Oktober 2010) Ordinance on Biocide Products
Regulation (EU) No 528/2012 of the European
Eco-Institute (2020) Parliament and of the Council of 22 May 2012
Test reports no. 55493­C006, 55493­C006 II and concerning the making available on the market and
55493­C006 III use of biocidal products.
European Waste code Umwelt Bundesamt 2021
in accordance with the European Waste Catalogue Umwelt Bundesamt: Herkunftsnachweisregister
(EWC) (EWC 2014/955/EU) Commission Decision (HKNR) — Entwertungsnachweis durch GETECH
amending Decision 2000/532/EC on the list of waste ENERGIE GMBH für HILTI
pursuant to Directive 2008/98/EC of the European
Parliament and of the Council
ETA-10/0109 Database
European Technical Approval Hilti CFS­F­FX
Ecoinvent 3.8
French VOC Directives ecoinvent Version 3
Décret no 2011­321 du 23 mars 2011 relatif à Wernet, G., Bauer, C., Steubing, B., Reinhard, J.,
l’étiquetage des produits de construction ou de Moreno­Ruiz, E., and Weidema, B., 2016. The
revêtement de mur ou de sol et des peintures et vernis ecoinvent database version 3 (part I): overview and
sur leurs émissions de polluants volatils methodology. The International Journal of Life Cycle
Arrêté du 19 avril 2011 relatif à l’étiquetage des Assessment, [online] 21(9), pp.1218–1230. Available
produits de construction ou de revêtement de mur ou at: <http://link.springer.com/10.1007/s11367­016­1087­
de sol et des peintures et vernis sur leurs émissions de 8> [Accessed in 2021/2022].
polluants volatils
ICC ESR-4878
International code council (ICC), Evaluation report
ESR­4878 HILTI HIT­HY 200 V3 (November 2021)
ICC ESR-4868
International code council (ICC), Evaluation report
ESR­4868 HILTI HIT­HY 200 V3 (March 2022)
10 Environmental Product Declaration Hilti – Hilti CFS­F FX
Publisher
Institut Bauen und Umwelt e.V. Tel +49 (0)30 3087748­ 0
Hegelplatz 1 Fax +49 (0)30 3087748­ 29
10117 Berlin Mail info@ibu­epd.com
Germany Web www.ibu-epd.com
Programme holder
Institut Bauen und Umwelt e.V. Tel +49 (0)30 ­ 3087748­ 0
Hegelplatz 1 Fax +49 (0)30 – 3087748 ­ 29
10117 Berlin Mail info@ibu­epd.com
Germany Web www.ibu-epd.com
Author of the Life Cycle
Assessment Tel +33 (0)9 53 23 98 30
ESTEANA Fax ­
Rue Mège 26 Mail contact@esteana.fr
83220 Le Pradet Web www.esteana.fr
France
Owner of the Declaration
Hilti Aktiengesellschaft Tel +423 234 2111
Feldkircher Strasse 100 Fax +423 234 2965
9494 Schaan Mail HAGHSE@hilti.com
Liechtenstein Web www.hilti.com
