ENVIRONMENTAL PRODUCT DECLARATION
as per ISO 14025 and EN 15804+A2
Owner of the Declaration Kuraray Europe GmbH
Publisher Institut Bauen und Umwelt e.V. (IBU)
Programme holder Institut Bauen und Umwelt e.V. (IBU)
Declaration number EPD-KUR-20230073-CBA2-EN
Issue date 12.03.2024
Valid to 11.03.2029
Ionoplast film (SentryGlas®) interlayer
Kuraray Europe GmbH
www.ibu-epd.com | https://epd-online.com
General Information
Kuraray Europe GmbH Ionoplast film (SentryGlas®) interlayer
Programme holder Owner of the declaration
IBU – Institut Bauen und Umwelt e.V. Kuraray Europe GmbH
Hegelplatz 1 Philipp-Reis-Str. 4
10117 Berlin 65795 Hattersheim
Germany Germany
Declaration number Declared product / declared unit
EPD-KUR-20230073-CBA2-EN The declared product is 1 m2 SentryGlas® with a density of 0.97 g/cm3.
This declaration is based on the product category rules: Scope:
Plate glass for construction and interlayers, 01.08.2021 SentryGlas® produced in Holesov, Czech Republic. Primary data of
(PCR checked and approved by the SVR) SentryGlas® production corresponds to the reference year 2020.
The owner of the declaration shall be liable for the underlying information
and evidence; the IBU shall not be liable with respect to manufacturer
Issue date information, life cycle assessment data and evidences.
12.03.2024
The EPD was created according to the specifications of EN 15804+A2. In
the following, the standard will be simplified as EN 15804.
Valid to
Verification
11.03.2029
The standard EN 15804 serves as the core PCR
Independent verification of the declaration and data according to ISO
14025:2011
internally X externally
Dipl.-Ing. Hans Peters
(Chairman of Institut Bauen und Umwelt e.V.)
Florian Pronold Dr. Matthew Fishwick,
(Managing Director Institut Bauen und Umwelt e.V.) (Independent verifier)
1 Environmental Product Declaration - Kuraray Europe GmbH - Ionoplast film (SentryGlas®) interlayer
Product
Name Value Unit
Product description/Product definition
Refractive index acc. to DIN EN ISO 489 1.49 -
SentryGlas® films are safety interlayers used in laminated
Thermal conductivity acc. to DIN EN 993-15 0.26 W/(mK)
architectural safety glass. These SentryGlas® interlayers offer
Thermal expansion coefficient acc. to ISO
safety advantages by retaining dangerous shards in case of 0.00013 K-1
11359-2
glass breakage. They are commonly used safety glass
interlayers available worldwide. Specific heat capacity 1.5 kJ/kgK
This EPD covers SentryGlas® produced in Holseov, Czech Surface resistivity acc. to DIN 53482 1E+13 Ω
Republic. Product codes: SentryGlas®, SentryGlas® Xtra, Performance data of the product with respect to its
SentryGlas® translucent white. characteristics in accordance with the relevant technical
provision (no CE-marking).
For the use and application of the product, the respective
national provisions at the place of use apply; in Germany, for Base materials/Ancillary materials
example, the building codes of the federal states and the The main constituents of SentryGlas® interlayer are (in mass
corresponding national specifications. percentages):
-SentryGlas® Resin ~99 %
Application
-Additives <1 %
SentryGlas® interlayers need to be laminated between two
pieces of glass. 1) This product contains substances listed in the candidate list
This sandwich arrangement is called laminated safety glass (date: 17.01.2023) exceeding 0.1 percentage by mass: no
according to EN ISO 14449.
2) This product contains other Carcinogenic, Mutagenic,
Technical Data
Reprotoxic (CMR) substances in categories 1A or 1B which are
For calculating the light, solar and heat parameters of glazing
not on the candidate list, exceeding 0.1 percentage by mass:
specifically containing films from the Trosifol® & SentryGlas®
no
product range please go to: https://www.trosifol.com/winslt-tool/
3) Biocide products were added to this construction product or it
Sound Control data can be found here:
has been treated with biocide products (this then concerns a
https://www.trosifol.com/soundlab-ai/
treated product as defined by the (EU) Ordinance on Biocide
Products No. 528/2012): no
The following data are valid for SentryGlas®. Other product's
data can be found in our laminator brochure: Reference service life
https://www.trosifol.com/de/salessupport/downloads/produktbro The reference service life is typically determined by the glass
schueren/ and not by the interlayer.
Constructional data
LCA: Calculation rules
production site and the production processes of the products
Declared Unit under study. The impact of packaging materials is included.
This declaration refers to the declared unit of 1m² of Ionoplast
film. The grammage of the Ionoplast film is 0.7372 kg/m². Module A5:
Declared unit Treatment and disposal of packaging material. Credits for
potential avoided burdens due to energy substitution of
Name Value Unit
electricity and thermal energy generation are declared in
Declared unit 1 m2 module D and affect only the rate of primary material (no
Grammage 0.7372 kg/m2 secondary materials).
Layer thickness 0.00076 m
Module C1 to C4:
Density 0.97 g/cm3
The end-of-life scenarios are as follows:
• C1 - Deconstruction/demolition: Dismantling is manual
(no environmental burden).
System boundary
• C2 - Transport to treatment/disposal site: Average
The type of EPD is cradle-to-gate with options, modules C1–
transport distance from the demolition site to waste
C4, and module D (A1–A3, C, D and additional module A5).
treatment is assumed as 50 km to the landfill.
• C3 - Waste processing for reuse, recovery or recycling:
In the following section, a detailed description of the specific
No waste processing (no environmental burden).
system boundaries is given:
• C4 - Disposal: Ionoplast film is 100 % landfilled.
Module A1 to A3:
Module D:
For the thermal and electrical energy generated in Module A5
The product stage includes the provision of all materials,
due to the thermal treatment of packaging and product waste,
products and energy, as well as waste processing up to the
avoided burdens have been calculated by the inversion of the
end-of-waste state or disposal of final residues during the
electricity grid mix and thermal energy from natural gas, using
product stage. These modules consider the manufacturing of
European datasets.
system components/raw materials, the transport to the
2 Environmental Product Declaration - Kuraray Europe GmbH - Ionoplast film (SentryGlas®) interlayer
Basically, a comparison or an evaluation of EPD data is only
Geographic Representativeness possible if all the data sets to be compared were created
Land or region, in which the declared product system is according to EN 15804 and the building context, respectively
manufactured, used or handled at the end of the product´s the product-specific characteristics of performance, are taken
lifespan: Europe into account. Background datasets: LCA for Experts (formerly
GaBi software) 10.6 software and Managed LCA Content
(formerly GaBi Databases) version 2022.1.
Comparability
LCA: Scenarios and additional technical information
Characteristic product properties of biogenic carbon
End of life (C1-C4)
Biogenic carbon is only present in the packaging (wooden
The end-of-life scenarios are as follows:
pallets).
C1 – The deconstruction of the Ionoplast film is assumed to be
Assumed water content in wooden pallets (packaging): 18 %.
done manually. Therefore, no environmental loads for the
Assumed carbon content: dry wood mass consists of 50 %
dismantling of this product are considered.
biogenic carbon.
C2 – Transport to treatment/disposal site: Average transport
The biogenic carbon content of the packaging is: 0.1294 kg
distance from the demolition site to waste treatment is assumed
pallet/declared unit * 0.82 *0.5 kg C / kg pallet (abs. dry) =
as 50 km to landfill.
0.0531 kg C/declared unit.
Information on describing the biogenic Carbon Content at C4 – Disposal: The Ionoplast film is 100% landfilled.
factory gate
Name Value Unit
Name Value Unit
Collected as mixed construction waste 0.7372 kg
Biogenic carbon content in accompanying kg
0.0531 Landfilling 0.7372 kg
packaging C
Reuse, recovery and/or recycling potentials (D), relevant
Note: 1 kg of biogenic carbon is equivalent to 44/12 kg of CO .
2 scenario information
For the thermal and electrical energy generated in Module A5
due to the thermal treatment of packaging, avoided burdens
The following technical scenario information is required for the
have been calculated by the inversion of the electricity grid mix
declared modules.
and thermal energy from natural gas, using European datasets.
Installation into the building (A5)
The packaging material treatment and disposal are also
considered in module A5.
Name Value Unit
Output substances following waste treatment on
0.1379 kg
site (packaging material)
3 Environmental Product Declaration - Kuraray Europe GmbH - Ionoplast film (SentryGlas®) interlayer
LCA: Results
DESCRIPTION OF THE SYSTEM BOUNDARY (X = INCLUDED IN LCA; MND = MODULE OR INDICATOR NOT DECLARED; MNR
= MODULE NOT RELEVANT)
Benefits and
Construction loads beyond
Product stage Use stage End of life stage
process stage the system
boundaries
la ire ta m w a Ry lp p u s tro p s n a rT g n iru tc a fu n a M e h t m o rf tro p s n a rTe tis e h t o t e ta g y lb m e s s A e s U e c n a n e tn ia M ria p e R tn e m e c a lp e R tn e m h s ib ru fe R y g re n e la n o ita re p Oe s u re ta w la n o ita re p Oe s u n o itc u rts n o c -e Dn o itilo m e d tro p s n a rT g n is s e c o rp e ts a W la s o p s iD -e s u e R-y re v o c e R-g n ilc y c e Rla itn e to p
A1 A2 A3 A4 A5 B1 B2 B3 B4 B5 B6 B7 C1 C2 C3 C4 D
X X X MND X MND MND MNR MNR MNR MND MND X X X X X
RESULTS OF THE LCA - ENVIRONMENTAL IMPACT according to EN 15804+A2: 1 m² Ionoplast film (SentryGlas®) interlayer
Parameter Unit A1-A3 A5 C1 C2 C3 C4 D
GWP-total kg CO 2 eq 2.64E+00 2.2E-01 0 2.27E-03 0 5.22E-02 -7.45E-02
GWP-fossil kg CO 2 eq 2.83E+00 3.01E-02 0 2.28E-03 0 5.22E-02 -7.41E-02
GWP-biogenic kg CO 2 eq -1.9E-01 1.9E-01 0 0 0 0 -3.79E-04
GWP-luluc kg CO 2 eq 4.48E-04 2.01E-06 0 1.54E-05 0 2.54E-05 -8.15E-06
ODP kg CFC11 eq 6.25E-12 1.56E-14 0 2.24E-16 0 7.02E-14 -5.02E-13
AP mol H+ eq 5.41E-03 3.11E-05 0 7.5E-06 0 1.55E-04 -9.75E-05
EP-freshwater kg P eq 3.04E-06 4.54E-09 0 8.15E-09 0 9.75E-06 -1.02E-07
EP-marine kg N eq 1.73E-03 1.01E-05 0 3.42E-06 0 3.43E-05 -2.64E-05
EP-terrestrial mol N eq 1.89E-02 1.49E-04 0 3.83E-05 0 3.76E-04 -2.83E-04
kg NMVOC
POCP 5.08E-03 2.7E-05 0 6.74E-06 0 1.1E-04 -7.4E-05
eq
ADPE kg Sb eq 4.37E-05 4.21E-10 0 2.3E-10 0 3.62E-09 -1.12E-08
ADPF MJ 7.41E+01 4.84E-02 0 2.99E-02 0 7.41E-01 -1.26E+00
m3 world eq
WDP 7.22E-01 2.23E-02 0 2.55E-05 0 -5.15E-04 -7.9E-03
deprived
GWP = Global warming potential; ODP = Depletion potential of the stratospheric ozone layer; AP = Acidification potential of land and water; EP =
Eutrophication potential; POCP = Formation potential of tropospheric ozone photochemical oxidants; ADPE = Abiotic depletion potential for non-fossil
resources; ADPF = Abiotic depletion potential for fossil resources; WDP = Water (user) deprivation potential)
RESULTS OF THE LCA - INDICATORS TO DESCRIBE RESOURCE USE according to EN 15804+A2: 1 m² Ionoplast film
(SentryGlas®) interlayer
Parameter Unit A1-A3 A5 C1 C2 C3 C4 D
PERE MJ 9.01E+00 1.92E+00 0 2.07E-03 0 6.09E-02 -3.47E-01
PERM MJ 1.91E+00 -1.91E+00 0 0 0 0 0
PERT MJ 1.09E+01 1.03E-02 0 2.07E-03 0 6.09E-02 -3.47E-01
PENRE MJ 4.5E+01 4.32E-01 0 3.01E-02 0 3.06E+01 -1.26E+00
PENRM MJ 3.02E+01 -3.83E-01 0 0 0 -2.99E+01 0
PENRT MJ 7.52E+01 4.85E-02 0 3.01E-02 0 7.42E-01 -1.26E+00
SM kg 0 0 0 0 0 0 0
RSF MJ 0 0 0 0 0 0 0
NRSF MJ 0 0 0 0 0 0 0
FW m3 2.85E-02 5.25E-04 0 2.4E-06 0 9.6E-06 -3.33E-04
PERE = Use of renewable primary energy excluding renewable primary energy resources used as raw materials; PERM = Use of renewable primary
energy resources used as raw materials; PERT = Total use of renewable primary energy resources; PENRE = Use of non-renewable primary energy
excluding non-renewable primary energy resources used as raw materials; PENRM = Use of non-renewable primary energy resources used as raw
materials; PENRT = Total use of non-renewable primary energy resources; SM = Use of secondary material; RSF = Use of renewable secondary fuels;
NRSF = Use of non-renewable secondary fuels; FW = Use of net fresh water
RESULTS OF THE LCA – WASTE CATEGORIES AND OUTPUT FLOWS according to EN 15804+A2:
1 m² Ionoplast film (SentryGlas®) interlayer
Parameter Unit A1-A3 A5 C1 C2 C3 C4 D
HWD kg 3.84E-09 4.16E-12 0 1.59E-13 0 1.14E-10 -1.71E-10
NHWD kg 2.22E-02 1.49E-03 0 4.9E-06 0 7.34E-01 -6.37E-04
RWD kg 2.21E-03 2.55E-06 0 5.58E-08 0 9.11E-06 -9.94E-05
CRU kg 0 0 0 0 0 0 0
MFR kg 0 0 0 0 0 0 0
MER kg 0 0 0 0 0 0 0
EEE MJ 0 3.34E-01 0 0 0 0 0
EET MJ 0 5.98E-01 0 0 0 0 0
4 Environmental Product Declaration - Kuraray Europe GmbH - Ionoplast film (SentryGlas®) interlayer
HWD = Hazardous waste disposed; NHWD = Non-hazardous waste disposed; RWD = Radioactive waste disposed; CRU = Components for re-use;
MFR = Materials for recycling; MER = Materials for energy recovery; EEE = Exported electrical energy; EET = Exported thermal energy
RESULTS OF THE LCA – additional impact categories according to EN 15804+A2-optional:
1 m² Ionoplast film (SentryGlas®) interlayer
Parameter Unit A1-A3 A5 C1 C2 C3 C4 D
Disease
PM 7.28E-08 1.56E-10 0 4.43E-11 0 1.49E-09 -8.08E-10
incidence
IR kBq U235 eq 1.93E-01 4.17E-04 0 8.42E-06 0 1.34E-03 -1.68E-02
ETP-fw CTUe 2.33E+01 2.33E-02 0 2.12E-02 0 7.26E-01 -2.77E-01
HTP-c CTUh 8.04E-10 1.45E-12 0 4.37E-13 0 3.26E-11 -1.27E-11
HTP-nc CTUh 3.93E-08 5.19E-11 0 2.71E-11 0 2.73E-09 -4.88E-10
SQP SQP 3.19E+01 1.44E-02 0 1.27E-02 0 5.33E-02 -2.25E-01
PM = Potential incidence of disease due to PM emissions; IR = Potential Human exposure efficiency relative to U235; ETP-fw = Potential comparative
Toxic Unit for ecosystems; HTP-c = Potential comparative Toxic Unit for humans (cancerogenic); HTP-nc = Potential comparative Toxic Unit for humans
(not cancerogenic); SQP = Potential soil quality index
Disclaimer 1 – for the indicator 'Potential Human exposure efficiency relative to U235'. This impact category deals mainly with the
eventual impact of low-dose ionizing radiation on human health of the nuclear fuel cycle. It does not consider effects due to possible
nuclear accidents, occupational exposure or radioactive waste disposal in underground facilities. Potential ionizing radiation from the
soil, radon and from some construction materials is also not measured by this indicator.
Disclaimer 2 – for the indicators 'abiotic depletion potential for non-fossil resources', 'abiotic depletion potential for fossil resources',
'water (user) deprivation potential, deprivation-weighted water consumption', 'potential comparative toxic unit for ecosystems', 'potential
comparative toxic unit for humans – cancerogenic', 'Potential comparative toxic unit for humans - not cancerogenic', 'potential soil
quality index'. The results of this environmental impact indicator shall be used with care as the uncertainties on these results are high
as there is limited experience with the indicator.
References
Standards Authorisation, published on ECHA website, latest version
17.01.2023 (https://echa.europa.eu/candidatelist-table)
DIN 53482
DIN 53482:1967-01, Testing of Insulating Materials; LCA for Experts (formerly GaBi software)
Determination of Electrical Resistances Values. Software System and Database for Life Cycle Engineering,
1992-2021, Sphera Solutions GmbH, Leinfelden-Echterdingen,
DIN EN ISO 489 with acknowledgement of LBP University of Stuttgart, program
DIN EN ISO 489:1999-08, Plastics - Determination of the version 10; database version 2022.1.
refractive index (ISO 489:1999).
Managed LCA Content documentation (formerly GaBi
DIN EN 993-15 Databases)
DIN EN 993-15:2005-07, Methods of test for dense shaped Dataset documentation for the software system and databases,
refractory products - Part 15: Determination of thermal LBP, University of Stuttgart and Sphera Solutions GmbH,
conductivity by the hot-wire (parallel) method. Leinfelden-Echterdingen, 2021. (https://sphera.com/product-
sustainability-gabi-data-search/)
EN 15804
EN 15804:2012+A2:2019+AC:2021, Sustainability of IBU 2021
construction works Environmental Product Declarations Core Institut Bauen und Umwelt e.V.: General Instructions for the
rules for the product category of construction products. EPD programme of Institut Bauen und Umwelt e.V., Version
2.0, Berlin: Institut Bauen und Umwelt e.V., 2021 www.ibu-
EN ISO 14449 epd.com
EN 14449:2005/AC:2005, Glass in building - Laminated glass
and laminated safety glass - Evaluation of conformity/Product Ordinance on Biocide Products No. 528/2012
standard. Regulation (EU) No 528/2012 of the European Parliament and
of the Council of 22 May 2012 concerning the making available
ISO 11359-2 on the market and use of biocidal products
ISO 11359-2:2021-11, Plastics - Thermomechanical analysis
(TMA) - Part 2: Determination of coefficient of linear thermal PCR Part A
expansion and glass transition temperature. PCR Part A: Calculation rules for the Life Cycle Assessment
and Requirements on the Background Report according to EN
ISO 14025 15 804+A2:2019, Version 1.3, Institut Bauen und Umwelt e.V.,
EN ISO 14025:2011, Environmental labels and declarations 2020.
Type III environmental declarations Principles and procedures.
PCR Part B
Further References Product Category Rules for Building Products, Part B:
Requirements on the EPD for plate glass for construction and
Candidate list interlayers, version 1.6, 2022 www.bau-umwelt.de
Candidate List of substances of very high concern for
5 Environmental Product Declaration - Kuraray Europe GmbH - Ionoplast film (SentryGlas®) interlayer
Publisher
Institut Bauen und Umwelt e.V. +49 (0)30 3087748- 0
Hegelplatz 1 info@ibu-epd.com
10117 Berlin www.ibu-epd.com
Germany
Programme holder
Institut Bauen und Umwelt e.V. +49 (0)30 3087748- 0
Hegelplatz 1 info@ibu-epd.com
10117 Berlin www.ibu-epd.com
Germany
Author of the Life Cycle Assessment
Sphera Solutions GmbH +49 711 341817-0
Hauptstraße 111- 113 info@sphera.com
70771 Leinfelden-Echterdingen www.sphera.com
Germany
Owner of the Declaration
Kuraray Europe GmbH +49 69 305 85 300
Philipp-Reis-Str. 4 trosifol@kuraray.com
65795 Hattersheim https://www.kuraray.eu/
Germany
6 Environmental Product Declaration - Kuraray Europe GmbH - Ionoplast film (SentryGlas®) interlayer
