ENVIRONMENTAL PRODUCT DECLARATION
as per ISO 14025 and EN 15804+A2
Owner of the Declaration danfloor a/s
Publisher Institut Bauen und Umwelt e.V. (IBU)
Programme holder Institut Bauen und Umwelt e.V. (IBU)
Declaration number EPD-DAN-20240101-CBA1-EN
Issue date 29.11.2024
Valid to 28.11.2029
Woven wall-to-wall carpet, 95 % recycled polyamide 6 with total
pile weight of 630 g/m2 and a textile backing
danfloor a/s
www.ibu-epd.com | https://epd-online.com
General Information
danfloor a/s Woven wall-to-wall carpet, 95 % recycled
polyamide 6 with total pile weight of 630 g/m2 and
a textile backing
Programme holder Owner of the declaration
IBU – Institut Bauen und Umwelt e.V. danfloor a/s
Hegelplatz 1 Østerbro 9
10117 Berlin 6933 Kibæk
Germany Denmark
Declaration number Declared product / declared unit
EPD-DAN-20240101-CBA1-EN 1 m² Woven wall-to-wall carpet, PA 6 pile material with a SBR based textile
backing
This declaration is based on the product category rules: Scope:
Floor coverings, 01.08.2021 The manufacturer declaration applies to a woven wall-to-wall carpet with a
(PCR checked and approved by the SVR) SBR based textile backing, a pile material of 95 % recycled PA 6 with a
total pile weight of 630 g/m2. The products are produced and coated in
Bording, Denmark.
Issue date The declaration is only valid in conjunction with a valid GUT-PRODIS
license of the product.
29.11.2024
The owner of the declaration shall be liable for the underlying information
and evidence; the IBU shall not be liable with respect to manufacturer
information, life cycle assessment data and evidences.
Valid to
28.11.2029 The EPD was created according to the specifications of EN 15804+A2. In
the following, the standard will be simplified as EN 15804.
Verification
The standard EN 15804 serves as the core PCR
Independent verification of the declaration and data according to ISO
14025:2011
internally X externally
Dipl.-Ing. Hans Peters
(Chairman of Institut Bauen und Umwelt e.V.)
Florian Pronold Angela Schindler,
(Managing Director Institut Bauen und Umwelt e.V.) (Independent verifier)
1 Environmental Product Declaration - danfloor a/s - Woven wall-to-wall carpet, 95 % recycled polyamide 6 with total pile weight of 630 g/m2 and a textile backing
Product
Additional product properties in accordance with EN 1307 can
Product description/Product definition be found on the Product Information System PRODIS using the
The declaration applies to a woven wall-to-wall carpet having a PRODIS registration number of the product (www.pro-dis.info)
surface pile of 95 % recycled solution-dyed polyamide 6 with a or on the manufacturer's technical information section.
total pile weight of 630 g/m2. The backing of the carpet consists
of a Styrene-Butadiene-Rubber (SBR) based textile backing. Base materials/Ancillary materials
The total recycled content of the carpet is 25 %. For the placing Name Value Unit
on the market of the specific product in the European Polyamide 6 26.4 %
Union/European Free Trade Association (EU/EFTA) (with the
Polypropylene 6.1 %
exception of Switzerland) Regulation (EU) No. 305/2011
Polyester 15,9 %
Construction Product Regulation (CPR) applies. The product
needs a Declaration of Performance (DoP) taking into Polymer dispersion 11,7 %
consideration EN 14041:2018-05, Resilient, textile and laminate Limestone 27,4 %
floor coverings - Essential characteristics, and the CE-marking. ATH 11,8 %
The DoP of the product can be found on the manufacturer's
Additives 0,7 %
technical information section. For the application and use of the
product the respective national provisions apply. The specific product covered by the EPD contains substances
listed in the ECHA candidate list (14.06.2023) or other
Application carcinogenic, mutagenic or reprotoxic (CMR) substances in
The use class of the specific product as defined in EN 1307 can categories 1A or 1B which are not on the candidate list
be found in the Product Information System (PRODIS) using exceeding 0.1 percentage by mass: no
the PRODIS registration number of the product. The products are registered in the GUT-PRODIS Information
System. The PRODIS system ensures compliance with
Technical Data limitations of various chemicals and Volatile Organic
Compounds (VOC)-emissions and a ban on the use of all
Constructional data according to EN 1307 substances that are listed as 'Substances of Very High
Concern' (SVHC) under REACH.
Name Value Unit
Product Form Wall-to-wall carpet on rolls - Reference service life
Type of manufacture Woven carpet - The service life of textile floor coverings strongly depends on
Yarn type Polyamide 6 - the correct installation taking into account the declared use
classification and the adherence to cleaning and maintenance
Total carpet weight 2400 g/m2
instructions.
Secondary backing SBR based textile backing - A calculation of the reference service life according to ISO
Performance data of the product in accordance with the 15686 is not possible. Alternatively, a reference service life of
declaration of performance with respect to its essential 10 years can be assumed, during which the functional and
characteristics according to EN 14041: 2018-05, Resilient, visual quality is guaranteed (BNB, Nutzungsdauer von
textile and laminate floor coverings - Essential characteristics. Bauteilen). The technical service life can be significantly longer.
LCA: Calculation rules
Declared Unit A1-A3 Production:
Energy supply and production of the basic material, processing
Name Value Unit of secondary material, auxiliary material, transport of the
Declared unit 1 m2 material to the manufacturing site, emissions, waste water
treatment, packaging material and waste processing up to the
Grammage 2.4 kg/m2
landfill disposal of residual waste (except radioactive waste).
Layer thickness 0.004 m Benefits for generated electricity and steam due to the
Gross density 595 kg/m3 incineration of production waste are aggregated.
The declared unit refers to 1 m2 produced textile floor covering.
A4 Transport:
The Output of module A5 'Assembly' is 1 m2 installed textile
Transport of the packed textile floor covering from factory gate
floor covering.
to the place of installation.
A5 Installation:
Installation of the textile floor covering, processing of
System boundary
installation waste and packaging waste up to the landfill
Type of EPD: Cradle-to-grave
disposal of residual waste (except radioactive waste), the
System boundaries of modules A, B, C, D:
production of the amount of carpet that occurs as installation
waste including its transport to the place of installation.
Generated electricity and steam due to the incineration of
Modules C3, C4 and D are indicated separately for three end-
waste are listed in the result table as exported energy.
of-life scenarios:
Biogenic carbon that is stored in renewable materials in
0 - landfill disposal
packaging paper is released as carbon dioxide emissions into
1 - municipal waste incineration
the air at the end of life in module A5. Preparation of the floor
2 - recovery in a cement plant
and auxiliary materials (adhesives, fixing agents, PET
2 Environmental Product Declaration - danfloor a/s - Woven wall-to-wall carpet, 95 % recycled polyamide 6 with total pile weight of 630 g/m2 and a textile backing
connectors) are beyond the system boundaries and not taken exported energy.
into account. C3-2: Collection of the carpet waste for recovery in the cement
industry, waste processing (granulating), transport to the
B1 Use: cement plant, emissions from the incineration.
Indoor emissions during the use stage. After the first year, no
product-related Volatile Organic Compound (VOC) emissions C4 Disposal
are relevant due to known VOC decay curves of the product. C4: Impact from landfill disposal,
C4-1: The carpet waste leaves the system in module C3-2,
B2 Maintenance: C4-2: The pre-processed carpet waste leaves the system in
Cleaning of the textile floor covering for a period of 1 year: module C3-3.
Vacuum cleaning – electricity supply
Wet cleaning – electricity, water consumption, production of the D Recycling potential:
cleaning agent, waste water treatment. Calculated benefits result from materials exclusive secondary
The declared values in this module have to be multiplied by the materials (net materials).
assumed service life of the floor covering in the building in D: Benefits for generated energy due to landfill disposal of
question. carpet waste at the end-of-life,
D-1: Benefits for generated energy due to incineration of carpet
B3 - B5: waste at the end-of-life (incineration plant with R1 > 0.6),
The modules are not relevant within the assumed reference D-2: Benefits for saved fossil energy and saved inorganic
service life of 10 years. material due to recovery of the carpet in a cement plant.
D-3: Benefits for generated energy due to incineration of
B6 - B7: packaging and
No energy and water input are required for the operation of the installation waste (incineration plant with R1 > 0.6).
carpet in the use stage. The modules do not cause an
environmental impact. Geographic Representativeness
Land or region, in which the declared product system is
C1 De-construction: manufactured, used or handled at the end of the product´s
The floor covering is de-constructed manually and no additional lifespan: Europe
environmental impact is caused.
Comparability
C2 Transport:
Basically, a comparison or an evaluation of EPD data is only
Transport of the carpet waste to a landfill, to the municipal
possible if all the data sets to be compared were created
waste incineration plant (MWI) or to the waste collection facility
according to EN 15804 and the building context, respectively
for recycling.
the product-specific characteristics of performance, are taken
into account. Background data are taken from the Sphera MLC
C3 Waste processing:
database 2023-2. Remaining data gaps are covered by the
C3: Landfill disposal needs no waste processing.
ecoinvent 3.9.
C3-1: Impact from waste incineration (plant with R1 > 0.6),
generated electricity and steam are listed in the result table as
LCA: Scenarios and additional technical information
Preparation of the floor and auxiliaries (adhesives, fixing
Characteristic product properties of biogenic carbon agents, PET connectors etc.) are not taken into account.
Name ValueUnit
Maintenance (B2)
Biogenic carbon content in product at factory gate - kg The values for cleaning refer to 1 m2 floor covering per year.
C
Depending on the application based on ISO 10874, the
Biogenic carbon content in accompanying kg technical service life recommended by the manufacturer and
0.018
packaging at factory gate C the anticipated strain on the floor by customers, the case-
1 kg biogenic Carbon is equivalent to 44/12 kg of CO specific useful life can be established. Based on this useful life
2
the effects of module B2 need to be calculated in order to
obtain the overall environmental impacts.
Name Value Unit
Maintenance cycle (vacuum cleaning) 208 Number /year
Transport to the construction site (A4) Maintenance cycle (wet cleaning) 1,5 Number /year
Name Value Unit Water consumption (wet cleaning) 0.004 m3
Litres of fuel (truck, EURO 0-6 mix) 0.0066 l/100km Cleaning agent (wet cleaning) 0.09 kg
Transport distance 700 km Electricity consumption 0.314 kWh
Capacity utilisation (including empty runs) 55 % For further information on cleaning and maintenance see
www.danfloor.com
Installation in the building (A5)
Name Value Unit
Material loss 0.215 kg Service life
Polyethylene packaging waste and installation waste are
considered to be incinerated in a municipal waste incineration
plant. Cardboard packaging waste is going to be recycled.
3 Environmental Product Declaration - danfloor a/s - Woven wall-to-wall carpet, 95 % recycled polyamide 6 with total pile weight of 630 g/m2 and a textile backing
Name Value Unit should be done according to the following scheme:
EOL-impact = x % impact (Scenario 0)
Life Span (according to BBSR) 10 a
+ y % impact (Scenario 1)
Corresponds to the
Declared product properties (at + z % impact (Scenario 2)
specifications of EN -
the gate) and finishes with x % + y % + z % = 100 %
1307
Name ValueUnit
An assumed quality of work,
w wh ithe n
th
i en s mta all ne ud
f
ain
c
ta uc reco r’r sdance C mo an nfo ur fm acs t uto re t rh 'se - C ano dll e 1c )ted as mixed construction waste (scenarios 0 2.383 kg
instructions
instructions Collected separately waste type (scenario 2) 2.383 kg
Usage conditions, e.g. Use in areas defined by Landfilling (scenario 0) 2.383 kg
frequency of use, mechanical the use class according - Energy recovery (scenario 1) 2.383 kg
exposure to EN 1307
Energy recovery (scenario 2) 1.447 kg
Maintenance e.g. required According to the
Recycling (scenario 2) 0.933 kg
frequency, type and quality and manufacturers -
replacement of components instructions
Reuse, recovery and/or recycling potentials (D), relevant
End of Life (C1-C4) scenario information
Three different end-of-life scenarios are declared and the Recovery or recycling potentials due to the three end-of-life
results are indicated separately in module C. scenarios (module C) are indicated separately.
Each scenario is calculated as a 100% scenario.
Recycling in the cement industry (scenario 3):
Scenario 0: 100 % landfill disposal The organic material of the carpet is used as an alternative fuel
Scenario 1: 100 % municipal waste incineration (MWI) in a cement kiln. It mainly substitutes for lignite (68.8 %), hard
with R1>0.6 coal (23.6 %) and petrol coke (7.6 %). The inorganic material is
Scenario 2: 100 % recovery in the cement industry substantially integrated into the cement clinker and substitutes
for original material input. VDZ e.V.
If combinations of these scenarios have to be calculated this
4 Environmental Product Declaration - danfloor a/s - Woven wall-to-wall carpet, 95 % recycled polyamide 6 with total pile weight of 630 g/m2 and a textile backing
LCA: Results
The declared result figures in module B2 have to be multiplied by the assumed service life (in years) of the floor covering in the building
under consideration. Information on un-declared modules: Modules B3 - B7 are not relevant during the service life of the carpet and are
therefore not declared. Modules C1, C3, C4/1 and C4/2 cause no additional impact (see "LCA: Calculation rules") and are therefore not
declared. Module C2 represents the transport for scenarios 0, 1 and 2. Column D/3 represents module D/A5.
Version number of the characterisation factors used : EN 15804+A2 (based on EF 3.1)
DESCRIPTION OF THE SYSTEM BOUNDARY (X = INCLUDED IN LCA; MND = MODULE OR INDICATOR NOT DECLARED; MNR
= MODULE NOT RELEVANT)
Benefits and
Construction loads beyond
Product stage Use stage End of life stage
process stage the system
boundaries
la ire ta m w a Ry lp p u s tro p s n a rT g n iru tc a fu n a M e h t m o rf tro p s n a rTe tis e h t o t e ta g y lb m e s s A e s U e c n a n e tn ia M ria p e R tn e m e c a lp e R tn e m h s ib ru fe R y g re n e la n o ita re p Oe s u re ta w la n o ita re p Oe s u n o itc u rts n o c -e Dn o itilo m e d tro p s n a rT g n is s e c o rp e ts a W la s o p s iD -e s u e R-y re v o c e R-g n ilc y c e Rla itn e to p
A1 A2 A3 A4 A5 B1 B2 B3 B4 B5 B6 B7 C1 C2 C3 C4 D
X X X X X X X MNR MNR MNR MND MND X X X X X
RESULTS OF THE LCA - ENVIRONMENTAL IMPACT according to EN 15804+A2: 1 m² floor covering
Parameter Unit A1-A3 A4 A5 B1 B2 C1 C2 C3 C3/1 C3/2 C4 C4/1 C4/2 D D/1 D/2 D/3
GWP-total kg CO 2 5.68E 1.78E- 8.44E- 0 5.15E- 0 9.77E- 0 3.46E 3.5E 1.62E- 0 0 0 -5.33E- -1.94E- -4.79E-
eq +00 01 01 01 03 +00 +00 01 01 01 02
GWP-fossil kg CO 2 5.72E 1.76E- 8.43E- 0 3.15E- 0 9.66E- 0 3.46E 3.5E 1.62E- 0 0 0 -5.3E-01 -1.94E- -4.77E-
eq +00 01 01 01 03 +00 +00 01 01 02
GWP- kg CO 2 -4.5E- 4.11E- 6.46E- 0 3.69E- 0 2.26E- 0 2.91E- 4.4E-04 0 0 0 0 -2.39E- -1.41E- -2.15E-
biogenic eq 02 04 05 03 05 04 03 04 04
GWP-luluc kg CO 2 5.59E- 1.66E- 6.68E- 0 1.96E- 0 9.14E- 0 1.01E- 3.31E- 1.35E- 0 0 0 -3.42E- -1.23E- -3.08E-
eq 03 03 04 01 05 04 04 04 05 04 06
kg
6.92E- 1.57E- 6.23E- 3.42E- 8.64E- 3.07E- 5.06E- 2.75E- -4.09E- -2.68E- -3.68E-
ODP CFC11 0 0 0 0 0 0
09 14 10 08 16 13 13 13 12 13 13
eq
mol H+ 1.38E- 1.62E- 7.94E- 6.08E- 3.05E- 3.22E- 4.92E- -6.57E- -5.91E-
AP 1.1E-03 0 0 0 0 0 0 -8.6E-04
eq 02 03 04 05 03 03 04 04 05
EP- 4.73E- 6.54E- 4.35E- 5.23E- 3.84E- 5.14E- 3.15E- -8.43E- -2.61E- -7.59E-
kg P eq 0 0 3.6E-08 0 0 0 0
freshwater 05 07 06 06 07 07 05 07 07 08
4.79E- 5.41E- 6.15E- 1.92E- 2.98E- 1.49E- 1.57E- 1.13E- -1.93E- -2.52E- -1.74E-
EP-marine kg N eq 0 0 0 0 0 0
03 04 04 04 05 03 03 04 04 04 05
2.77E- 1.67E- 1.76E- 1.24E- -2.07E- -2.76E- -1.86E-
EP-terrestrial mol N eq 4.6E-02 6E-03 6.2E-03 0 0 3.3E-04 0 0 0 0
03 02 02 03 03 03 04
kg
1.28E- 1.02E- 1.59E- 4.18E- 9.67E- 5.63E- 3.82E- 3.98E- 3.58E- -5.38E- -7.42E- -4.84E-
POCP NMVOC 0 0 0 0 0
02 03 03 04 04 05 03 03 04 04 04 05
eq
1.53E- 1.17E- 1.39E- 2.14E- 6.41E- 8.61E- 1.19E- 4.33E- -3.74E- -1.37E- -3.37E-
ADPE kg Sb eq 0 0 0 0 0 0
06 08 07 07 10 09 08 09 08 08 09
1.25E 2.44E 1.16E 5.93E 1.34E- 1.69E 2.25E 2.45E -9.77E -2.04E
ADPF MJ 0 0 0 0 0 0 -8.8E-01
+02 +00 +01 +00 01 +00 +00 +00 +00 +01
m3 world
3.94E 2.07E- 3.92E- 9.61E- 1.14E- 4.21E- 4.23E- -2.31E- -4.95E- -2.27E- -4.46E-
WDP eq 0 0 0 0 0 0
+00 03 01 02 04 01 01 03 02 02 03
deprived
GWP = Global warming potential; ODP = Depletion potential of the stratospheric ozone layer; AP = Acidification potential of land and water; EP =
Eutrophication potential; POCP = Formation potential of tropospheric ozone photochemical oxidants; ADPE = Abiotic depletion potential for non-fossil
resources; ADPF = Abiotic depletion potential for fossil resources; WDP = Water (user) deprivation potential)
RESULTS OF THE LCA - INDICATORS TO DESCRIBE RESOURCE USE according to EN 15804+A2: 1 m² floor covering
Parameter Unit A1-A3 A4 A5 B1 B2 C1 C2 C3 C3/1 C3/2 C4 C4/1 C4/2 D D/1 D/2 D/3
4.98E 1.73E- 4.78E 3.79E 2.94E- 4.52E- 2.21E- -2.79E -3.48E- -2.51E-
PERE MJ 0 0 9.5E-03 0 0 0 0
+01 01 +00 +00 01 01 01 +00 01 01
2.34E- -2.34E-
PERM MJ 0 0 0 0 0 0 0 0 0 0 0 0 0 0 0
01 01
1.73E- 4.55E 3.79E 2.94E- 4.52E- 2.21E- -2.79E -3.48E- -2.51E-
PERT MJ 5E+01 0 0 9.5E-03 0 0 0 0
01 +00 +00 01 01 01 +00 01 01
1.01E 2.45E 1.37E 5.93E 1.35E- 2.33E 2.39E 2.45E -9.78E -2.04E
PENRE MJ 0 0 0 0 0 0 -8.8E-01
+02 +00 +01 +00 01 +01 +01 +00 +00 +01
2.38E -2.12E -2.16E -2.16E
PENRM MJ 0 0 0 0 0 0 0 0 0 0 0 0 0
+01 +00 +01 +01
1.25E 2.45E 1.16E 5.93E 1.35E- 1.69E 2.25E 2.45E -9.78E -2.04E
PENRT MJ 0 0 0 0 0 0 -8.8E-01
+02 +00 +01 +00 01 +00 +00 +00 +00 +01
5 Environmental Product Declaration - danfloor a/s - Woven wall-to-wall carpet, 95 % recycled polyamide 6 with total pile weight of 630 g/m2 and a textile backing
6.62E-
SM kg 0 5.96E-02 0 0 0 0 0 0 0 0 0 0 0 0 5.5E-01 0
01
RSF MJ 0 0 0 0 0 0 0 0 0 0 0 0 0 0 0 0 0
NRSF MJ 0 0 0 0 0 0 0 0 0 0 0 0 0 0 0 0 0
9.67E- 3.26E- 1.05E- 9.94E- 1.01E- 2.41E- -2.26E- -1.98E- -2.03E-
FW m3 1.9E-04 9.61E-03 0 0 0 0 0 0
02 03 05 03 02 05 03 03 04
PERE = Use of renewable primary energy excluding renewable primary energy resources used as raw materials; PERM = Use of renewable primary
energy resources used as raw materials; PERT = Total use of renewable primary energy resources; PENRE = Use of non-renewable primary energy
excluding non-renewable primary energy resources used as raw materials; PENRM = Use of non-renewable primary energy resources used as raw
materials; PENRT = Total use of non-renewable primary energy resources; SM = Use of secondary material; RSF = Use of renewable secondary fuels;
NRSF = Use of non-renewable secondary fuels; FW = Use of net fresh water
RESULTS OF THE LCA – WASTE CATEGORIES AND OUTPUT FLOWS according to EN 15804+A2:
1 m² floor covering
Parameter Unit A1-A3 A4 A5 B1 B2 C1 C2 C3 C3/1 C3/2 C4 C4/1 C4/2 D D/1 D/2 D/3
1.75E- 9.05E- 1.58E- 4.19E- 4.98E- 2.04E- 1.88E- 2.06E- -5.44E- -1.61E- -4.89E-
HWD kg 0 0 0 0 0 0
03 12 04 05 13 10 10 10 10 10 11
4.54E- 3.53E- 8.45E- 7.29E- 1.94E- 4.84E- 4.84E- 2.37E -4.78E- -1.33E- -4.31E-
NHWD kg 0 0 0 0 0 0
01 04 02 03 05 01 01 +00 03 01 04
2.12E- 3.16E- 1.97E- 3.79E- 1.74E- 6.12E- 9.74E- -6.66E-
RWD kg 0 0 0 2.9E-05 0 0 0 -7.4E-04 -7.4E-05
03 06 04 04 07 05 05 05
CRU kg 0 0 0 0 0 0 0 0 0 0 0 0 0 0 0 0 0
1.56E-
MFR kg 0 1.4E-03 0 0 0 0 0 0 5.5E-01 0 0 0 0 0 0 0
02
MER kg 0 0 0 0 0 0 0 0 0 0 0 0 0 0 0 0 0
5.12E
EEE MJ 0 0 4.6E-01 0 0 0 0 0 0 0 0 0 0 0 0 0
+00
8.41E- 9.34E 4.08E
EET MJ 0 0 0 0 0 0 0 0 0 0 0 0 0 0
01 +00 +01
HWD = Hazardous waste disposed; NHWD = Non-hazardous waste disposed; RWD = Radioactive waste disposed; CRU = Components for re-use;
MFR = Materials for recycling; MER = Materials for energy recovery; EEE = Exported electrical energy; EET = Exported thermal energy
RESULTS OF THE LCA – additional impact categories according to EN 15804+A2-optional:
1 m² floor covering
Parameter Unit A1-A3 A4 A5 B1 B2 C1 C2 C3 C3/1 C3/2 C4 C4/1 C4/2 D D/1 D/2 D/3
Disease 1.05E- 6.95E- 1.12E- 6.82E- 3.82E- 1.22E- 1.34E- 4.77E- -1.71E- -5.01E-
PM 0 0 0 0 0 0 0
incidence 07 09 08 08 10 08 08 09 08 10
kBq U235 3.48E- 4.57E- 3.22E- 6.73E- 2.51E- 9.34E- 1.53E- 4.29E- -9.37E- -1.11E-
IR 0 0 0 0 0 0 0
eq 01 04 02 02 05 03 02 03 03 02
4.48E 1.72E 4.26E 3.6E- 2.07E 9.46E- 6.94E- 9.93E- 2.09E -7.79E
ETP-fw CTUe 0 0 0 0 0 0 -1.2E-01
+01 +00 +00 03 +00 02 01 01 +00 +00
2.86E- 3.48E- 2.64E- 6.26E- 1.91E- 5.01E- 1.07E- -5.93E- -9.68E-
HTP-c CTUh 0 0 0 4.2E-11 0 0 0 0
09 11 10 10 12 11 10 11 12
1.02E- 1.53E- 2.6E- 6.16E- 8.43E- 2.26E- 8.56E- -3.23E-
HTP-nc CTUh 9.5E-09 0 0 2E-09 0 0 0 0 -2.4E-10
07 09 11 09 11 09 09 09
SQP SQP ND ND ND ND ND 0 ND ND ND ND ND ND ND ND ND ND ND
PM = Potential incidence of disease due to PM emissions; IR = Potential Human exposure efficiency relative to U235; ETP-fw = Potential comparative
Toxic Unit for ecosystems; HTP-c = Potential comparative Toxic Unit for humans (cancerogenic); HTP-nc = Potential comparative Toxic Unit for humans
(not cancerogenic); SQP = Potential soil quality index
No substantiated values can be given for the SQP indicator with the existing database.
The result figures given in module B2 refer to a period of 1 year because a reference service life is not declared. They have to be
multiplied by the assumed service life (in years) of the floor covering in the building under consideration.
Disclaimer 1 – for the indicator 'Potential Human exposure efficiency relative to U235'. This impact category deals mainly with the
eventual impact of low-dose ionizing radiation on human health of the nuclear fuel cycle. It does not consider effects due to possible
nuclear accidents, occupational exposure or radioactive waste disposal in underground facilities. Potential ionizing radiation from the
soil, from radon and from some construction materials is also not measured by this indicator.
Disclaimer 2 – for the indicators 'abiotic depletion potential for non-fossil resources', 'abiotic depletion potential for fossil resources',
'water (user) deprivation potential, deprivation-weighted water consumption', 'potential comparative toxic unit for ecosystems', 'potential
comparative toxic unit for humans – cancerogenic', 'Potential comparative toxic unit for humans - not cancerogenic', 'potential soil
quality index'.
The results of this environmental impact indicator shall be used with care as the uncertainties on these results are high as there is
limited experience with the indicator.
References
EN 1307
DIN EN 1307: 2014+A1:2016+A2:2018-05: Textile floor EN 13501-1
coverings - Classification DIN EN 13501-1:2019-05: Fire classification of construction
6 Environmental Product Declaration - danfloor a/s - Woven wall-to-wall carpet, 95 % recycled polyamide 6 with total pile weight of 630 g/m2 and a textile backing
products and building elements - Part 1: Classification using General Instructions for the IBU-EPD Program
data from reaction to fire tests General Instructions for the EPD-Program of the Institut Bauen
und Umwelt e.V., The Preparation of Environmental Product
EN 14041 Declarations - EPDs, version 2.0, Institut Bauen und Umwelt
DIN EN 14041: 2018-05 and DIN EN 14041: 2008-05: e.V., Berlin, January 2021, www.ibu-epd.de
Resilient, textile and laminate floor coverings - Essential
characteristics BBSR
Bundesinstitut für Bau-, Stadt- und Raumforschung (BBSR) im
EN 15804 Bundesamt für Bauwesen und Raumordnung (BBR), Bonn
DIN EN
15804:2012+A2:2019+AC:2021, Sustainability of construction BNB, Nutzungsdauer von Bauteilen
works — Environmental Product Declarations — Core rules for Bewertungssystem Nachhaltiges Bauen (BNB), Nutzungsdauer
the product category of construction products von Bauteilen, Bundesministerium des Inneren, für Bau und
Heimat, 24.02.2017
EN 16810
DIN EN 16810: 2017-08: Resilient, textile and laminate floor ECHA candidate list
coverings – Environmental product declarations – Product Candidate
category rules List of substances of very high concern (SVHCs) for
authorisation,
ISO 10874 14.06.2023, European Chemicals Agency (ECHA), Helsinki,
DIN EN ISO 10874: 2012+A1:2021-04: Resilient, textile and Finland
laminate floor coverings - Classification
ecoinvent
ISO 14025 ecoinvent, Zurich, Switzerland, database version 3.9, published
DIN EN /ISO 14025:2011-10/, Environmental labels and September 2022
declarations — Type III environmental declarations —
Principles and procedures Sphera software and datanase
LCA FE software and MLC database for Life Cycle Engineering,
ISO 14040 Spehra Solutions Inc., Leinfelden-Echterdingen, 2023-2
DIN EN ISO 14040:2006+A1:2020 Environmental
management - Life cycle assessment - Principles and PCR Part A
framework Product Category Rules for Building-Related Products and
Services Part A: Calculation Rules for the Life Cycle
ISO 14044 Assessment and Requirements on the Project Report according
DIN EN ISO 14044:2006+A1:2018+A2:2020 Environmental to EN 15804+A2:2019, V1.3, Berlin: Institut Bauen und Umwelt
management - Life cycle assessment - Requirements and e.V. (IBU), August 2022
guidelines
PCR Part B
Product Category Rules for Building-Related Products and
ISO 15686 Services
ISO 15686: Buildings and constructed assets - Part B: Requirements on the EPD for floor coverings, v6, Berlin:
Service life planning Institut Bauen und Umwelt e.V. (IBU), June 2023
ISO 15686-1: 2011-05: Part 1: General principles and
framework PRODIS
ISO 15686-2: 2012-05: Part 2: Service life prediction Product Information System (PRODIS) of the European Carpet
procedures Industry, Gemeinschaft umweltfreundlicher Teppichboden e.V
ISO 15686-7: 2017-04: Part 7: Performance (GUT) and European Carpet and Rug Association (ECRA),
evaluation for feedback of service life data http://www.pro-dis.info
from practice
ISO 15686-8: 2008-06: Part 8: Reference service life REACH
and service-life estimation Regulation (EC) No 1907/2006 of the European Parliament and
of the Council of 18 December 2006 concerning the
Registration, Evaluation, Authorisation and Restriction of
Regulation (EU) No. 305/2011 Chemicals (REACH), June 2017, last update: 14.06.2023
Regulation No. 305/2011 Construction Products Regulation
(CPR) of the European Council and of the European VDZ e.V.
Parliament, April 2011 Association of German Cement Works, Ed. Environ-mental
Data of the German Cement Industry 2020
7 Environmental Product Declaration - danfloor a/s - Woven wall-to-wall carpet, 95 % recycled polyamide 6 with total pile weight of 630 g/m2 and a textile backing
Publisher
Institut Bauen und Umwelt e.V. +49 (0)30 3087748- 0
Hegelplatz 1 info@ibu-epd.com
10117 Berlin www.ibu-epd.com
Germany
Programme holder
Institut Bauen und Umwelt e.V. +49 (0)30 3087748- 0
Hegelplatz 1 info@ibu-epd.com
10117 Berlin www.ibu-epd.com
Germany
Author of the Life Cycle Assessment
Gemeinschaft umweltfreundlicher Teppichboden +49 (0)241 96843 410
(GUT) e.V. mail@gut-ev.de
Schönebergstraße 2 www.gut-ev.org
52068 Aachen
Germany
Owner of the Declaration
danfloor a/s +4596991900
Østerbro 9 sales@danfloor.com
6933 Kibæk www.danfloor.com
Denmark
8 Environmental Product Declaration - danfloor a/s - Woven wall-to-wall carpet, 95 % recycled polyamide 6 with total pile weight of 630 g/m2 and a textile backing
