ENVIRONMENTAL PRODUCT DECLARATION
as per ISO 14025 and EN 15804+A2
Owner of the Declaration dormakaba International Holding GmbH
Publisher Institut Bauen und Umwelt e.V. (IBU)
Programme holder Institut Bauen und Umwelt e.V. (IBU)
Declaration number EPD-DOR-20240260-CBA1-EN
Issue date 23.09.2024
Valid to 22.09.2029
Security Revolving Door Geryon K9
dormakaba
www.ibu-epd.com | https://epd-online.com
General Information
dormakaba Security Revolving Door Geryon K9
Programme holder Owner of the declaration
IBU – Institut Bauen und Umwelt e.V. dormakaba International Holding GmbH
Hegelplatz 1 DORMA Platz 1
10117 Berlin 58256 Ennepetal
Germany Germany
Declaration number Declared product / declared unit
EPD-DOR-20240260-CBA1-EN 1 piece of the product: Security Revolving Door Geryon K9, consisting of
the following items:
• Drive and control unit (K9)
• Upper body
• Side walls
• Door leafs
• Floor bearing
• Product packaging
This declaration is based on the product category rules: Scope:
Electronic and physical Access Control Systems, 01.08.2021 This Environmental Product Declaration refers to a specific security
(PCR checked and approved by the SVR) revolving door covering the variants 120° and 180°. The production site is
located in Bühl (Germany).
Green electricity with Guarantee of Origin (GoO) is being used at this
Issue date production site.
23.09.2024
Data represents the year 2024.
The owner of the declaration shall be liable for the underlying information
and evidence; the IBU shall not be liable with respect to manufacturer
Valid to
information, life cycle assessment data and evidences.
22.09.2029
The EPD was created according to the specifications of EN 15804+A2. In
the following, the standard will be simplified as EN 15804.
Verification
The standard EN 15804 serves as the core PCR
Independent verification of the declaration and data according to ISO
14025:2011
internally X externally
Dipl.-Ing. Hans Peters
(Chairman of Institut Bauen und Umwelt e.V.)
Florian Pronold Matthias Klingler,
(Managing Director Institut Bauen und Umwelt e.V.) (Independent verifier)
1 Environmental Product Declaration - dormakaba - Security Revolving Door Geryon K9
Product
Name Value Unit
Product description/Product definition
Outside diameter 1500-2000 mm
The Security Revolving Door Geryon K9 is characterized by a
Total height 2300 mm
high degree of transparency of the glass elements and a wide
variety of colors of the metal parts. All models blend elegantly Passage height 2100 mm
into the surroundings. Upper part of body 200 mm
A sensor system according to the latest standards prevents Number of door wings 3 or 4 pieces
injuries to the user. Depending on the security requirements,
Rotary cycle 120 or 180 °
the door can be equipped with a contact mat. Other variants
include reinforced bullet-and burglar-resistant versions that are Performance data of the product with respect to its
certified according to the RC2 and RC3 standards. Options like characteristics in accordance with the relevant technical
a rotary unit with emergency exit function or night lock complete provision which can be applied are mentioned above.
the product range.
For the Security Revolving Door the standards which can be
applied are the following:
Base materials/Ancillary materials
• Machinery Directive 2006/42/EC
The major material composition including the packaging is
• Directive 2014/30/EU
listed below:
• ROHS Directive 2011/65/EU
Name Value Unit
• EN 60335-2-103
• EN 61000 Glass 40 %
• EN 16005 Aluminum 32 %
• ISO 13849 Steel 20 %
• ISO 12100
Plastics 6 %
Electronics 1 %
The CE-marking takes into account the proof of conformity with
the respective harmonized standards based on the legal Paper 1 %
provisions above. For the application and use the respective The Security Revolving Door Geryon K9 includes partial articles
national provisions apply. which contain substances listed in the Candidate List of
REACH Regulation 1907/2006/EC (date: 23.01.2024)
Application
exceeding 0.1 percentage by mass: no
The Security Revolving Door Geryon K9 offers secure entry to:
• Sensitive areas The Candidate List can be found on the ECHA website
• Administrative buildings address: https://echa.europa.eu/de/home.
• Industrial premises
• Government agencies
• Ministries
• Banks and financial institutions
• Data and research centers
Reference service life
• Staff entrances at airports
• Nuclear power plants The reference service life of the Security Revolving Door is
about 20 years, depending on the application and frequency of
Technical Data use. For repairs and renewals, suitable spare parts are
The Security Revolving Door Geryon K9 has following technical available. The Security Revolving Door is tested and certified to
properties: EN 16005, meaning they are designed to withstand a minimum
of 2.000.000 cycles.
LCA: Calculation rules
— A1, raw material extraction, processing and mechanical
Declared Unit treatments, processing of secondary material input (e.g.
The declared unit is 1 piece of product: Security Revolving Door recycling processes),
Geryon K9 including packaging. — A2, transport to the manufacturer,
Name Value Unit — A3, manufacturing and assembly including provision of all
Declared unit 1 pce. materials, products and energy (green electricity with
Guarantee of Origin (GoO)), as well as waste processing up to
Mass of declared product without packaging 455,9 kg
the end-of-waste state.
Mass of packaging 3,65 kg
Construction stage - Modules A4-A5
The construction process stage includes:
System boundary — A4, transport to the building site;
Type of EPD: cradle to gate with options, modules — A5, installation into the building; including provision of all
C1–C4, and module D (A1–A3 + C + D and additional materials, products and energy, as well as waste processing up
modules: A4 + A5 + B6) to the end-of-waste state or disposal of final residues during the
construction
Production - Module A1-A3 process stage.
The product stage includes:
2 Environmental Product Declaration - dormakaba - Security Revolving Door Geryon K9
Use stage - Module B6 benefits.
The use stage related to the operation of the building includes:
— B6, operational energy use
Geographic Representativeness
End-of-life stage– Modules C1-C4 and D Land or region, in which the declared product system is
The end-of-life stage includes: manufactured, used or handled at the end of the product´s
— C1, de-construction, demolition: lifespan: Germany
— C2, transport to waste processing;
— C3, waste processing for reuse, recovery and/or recycling;
Comparability
— C4, disposal; including provision and all transport, provision
Basically, a comparison or an evaluation of EPD data is only
of all materials,
possible if all the data sets to be compared were created
products and related energy and water use.
according to EN 15804 and the building context, respectively
Module D (Benefits and loads beyond the system boundary)
the product-specific characteristics of performance, are taken
includes:
into account. GaBi, SP40.
— D, recycling potentials, expressed as net impacts and
LCA: Scenarios and additional technical information
Operational energy use (B6)
Characteristic product properties of biogenic carbon
Name Value Unit
Name ValueUnit Days per year in use 365 days
kg On mode per day 1 hours
Biogenic carbon content in product -
C Idle mode per day 15 hours
Biogenic carbon content in accompanying kg Off mode 8 hours
1.12
packaging C On mode power 56 W
Note: 1 kg of biogenic carbon is equivalent to 44/12 kg of CO . Idle mode power 12,4 W
2
Off mode power 0 W
Electricity consumption per 1 year 88,33 kWh
End of life (C1-C4)
Transport to the building site (A4) C1: The product dismantling from the building is done manually
without environmental burden.
Name Value Unit
C2: Transport to waste management is 50 km.
Litres of fuel (per 1 kg) 0.00276l/100km
Name Value Unit
Transport distance via medium truck 100 km
Collected separately waste type waste type 456 kg
Capacity utilisation (including empty runs) via
55 % Recycling 240 kg
medium truck
Energy recovery 27.3 kg
The product is transported via truck. The main distribution
Landfilling 189 kg
region is Europe. In order to allow scaling to a specific point of
installation 100 km is declared. The product is disassembled in a recycling process. Material
recycling is then assumed for the metals, and electronics. The
plastic components are assumed to be incinerated with energy
Installation into the building (A5)
recovery. Glass, electromechanics and batteries are assumed
Name Value Unit
to be landfilled. Region for the End of Life is: Global.
Waste packaging paper 3,05 kg
Waste packaging plastic 0,6 kg
Reuse, recovery and/or recycling potentials (D), relevant
scenario information
Reference service life Name Value Unit
Recycling 100 %
Name Value Unit
Life Span according to the manufacturer 20 a Collection rate is 100 %.
3 Environmental Product Declaration - dormakaba - Security Revolving Door Geryon K9
LCA: Results
DESCRIPTION OF THE SYSTEM BOUNDARY (X = INCLUDED IN LCA; MND = MODULE OR INDICATOR NOT DECLARED; MNR
= MODULE NOT RELEVANT)
Benefits and
Construction loads beyond
Product stage Use stage End of life stage
process stage the system
boundaries
la ire ta m w a Ry lp p u s tro p s n a rT g n iru tc a fu n a M e h t m o rf tro p s n a rTe tis e h t o t e ta g y lb m e s s A e s U e c n a n e tn ia M ria p e R tn e m e c a lp e R tn e m h s ib ru fe R y g re n e la n o ita re p Oe s u re ta w la n o ita re p Oe s u n o itc u rts n o c -e Dn o itilo m e d tro p s n a rT g n is s e c o rp e ts a W la s o p s iD -e s u e R-y re v o c e R-g n ilc y c e Rla itn e to p
A1 A2 A3 A4 A5 B1 B2 B3 B4 B5 B6 B7 C1 C2 C3 C4 D
X X X X X MND MND MNR MNR MNR X MND X X X X X
RESULTS OF THE LCA - ENVIRONMENTAL IMPACT according to EN 15804+A2: 1 piece SRD Geryon K9
Parameter Unit A1-A3 A4 A5 B6 C1 C2 C3 C4 D
GWP-total kg CO 2 eq 2.72E+03 4.02E+00 5.85E+00 7.15E+02 0 1.99E+00 6.96E+01 2.89E+00 -1.03E+03
GWP-fossil kg CO 2 eq 2.68E+03 3.84E+00 1.63E+00 7.11E+02 0 1.91E+00 6.95E+01 2.87E+00 -1.03E+03
GWP-biogenic kg CO 2 eq 3.13E+01 1.78E-01 4.22E+00 2.37E+00 0 8.8E-02 2.7E-02 1E-02 -3.03E+00
GWP-luluc kg CO 2 eq 9.27E-01 9.14E-05 1.57E-04 1.03E+00 0 4.54E-05 4E-03 8E-03 -1.65E-01
ODP kg CFC11 eq 5.59E-09 4.06E-16 1.55E-15 1.56E-11 0 2.01E-16 3.51E-14 1.06E-14 -7.24E-09
AP mol H+ eq 1.03E+01 4E-03 1E-03 1.57E+00 0 2E-03 1.2E-02 2.1E-02 -3.7E+00
EP-freshwater kg P eq 1.36E-03 8.22E-07 2.75E-07 2E-03 0 4.08E-07 5.59E-06 4.93E-06 -5.36E-04
EP-marine kg N eq 1.78E+00 1E-03 4.99E-04 3.49E-01 0 6.07E-04 3E-03 5E-03 -4.98E-01
EP-terrestrial mol N eq 1.97E+01 1.4E-02 7E-03 3.66E+00 0 7E-03 5.6E-02 5.8E-02 -5.38E+00
kg NMVOC
POCP 4.99E+00 3E-03 1E-03 9.55E-01 0 2E-03 8E-03 1.6E-02 -1.61E+00
eq
ADPE kg Sb eq 2E-02 1.15E-07 2.29E-08 2.06E-04 0 5.72E-08 4.81E-07 2.58E-07 -3E-03
ADPF MJ 3.61E+04 5.45E+01 2.07E+00 1.25E+04 0 2.7E+01 3.22E+01 3.76E+01 -1.42E+04
m3 world eq
WDP 2.29E+02 8E-03 6.92E-01 1.55E+02 0 4E-03 7.11E+00 3.01E-01 -5.32E+01
deprived
GWP = Global warming potential; ODP = Depletion potential of the stratospheric ozone layer; AP = Acidification potential of land and water; EP =
Eutrophication potential; POCP = Formation potential of tropospheric ozone photochemical oxidants; ADPE = Abiotic depletion potential for non-fossil
resources; ADPF = Abiotic depletion potential for fossil resources; WDP = Water (user) deprivation potential)
RESULTS OF THE LCA - INDICATORS TO DESCRIBE RESOURCE USE according to EN 15804+A2: 1 piece SRD Geryon K9
Parameter Unit A1-A3 A4 A5 B6 C1 C2 C3 C4 D
PERE MJ 8.5E+03 1.72E-01 3.7E+01 5.54E+03 0 8.5E-02 8.75E+00 4.93E+00 -6.18E+03
PERM MJ 3.7E+01 0 -3.66E+01 0 0 0 -3.62E-01 0 0
PERT MJ 8.53E+03 1.72E-01 4.32E-01 5.54E+03 0 8.5E-02 8.38E+00 4.93E+00 -6.18E+03
PENRE MJ 3.52E+04 5.45E+01 2.79E+01 1.25E+04 0 2.71E+01 9.35E+02 3.76E+01 -1.42E+04
PENRM MJ 9.28E+02 0 -2.58E+01 0 0 0 -9.02E+02 0 0
PENRT MJ 3.61E+04 5.45E+01 2.07E+00 1.25E+04 0 2.71E+01 3.22E+01 3.76E+01 -1.42E+04
SM kg 2.89E+01 0 0 0 0 0 0 0 0
RSF MJ 0 0 0 0 0 0 0 0 0
NRSF MJ 0 0 0 0 0 0 0 0 0
FW m3 2.01E+01 3.08E-04 1.6E-02 6.41E+00 0 1.53E-04 1.7E-01 9E-03 -1.11E+01
PERE = Use of renewable primary energy excluding renewable primary energy resources used as raw materials; PERM = Use of renewable primary
energy resources used as raw materials; PERT = Total use of renewable primary energy resources; PENRE = Use of non-renewable primary energy
excluding non-renewable primary energy resources used as raw materials; PENRM = Use of non-renewable primary energy resources used as raw
materials; PENRT = Total use of non-renewable primary energy resources; SM = Use of secondary material; RSF = Use of renewable secondary fuels;
NRSF = Use of non-renewable secondary fuels; FW = Use of net fresh water
RESULTS OF THE LCA – WASTE CATEGORIES AND OUTPUT FLOWS according to EN 15804+A2:
1 piece SRD Geryon K9
Parameter Unit A1-A3 A4 A5 B6 C1 C2 C3 C4 D
HWD kg 5.53E-05 5.29E-09 4.71E-09 5.18E-06 0 2.62E-09 1.23E-07 5.74E-07 -1.34E-04
NHWD kg 3.93E+02 6E-03 2.94E-01 8.87E+00 0 3E-03 7.22E+00 1.89E+02 -2.31E+02
RWD kg 1.23E+00 5.85E-05 9.8E-05 1.9E+00 0 2.9E-05 1E-03 4.28E-04 -1.48E+00
CRU kg 0 0 0 0 0 0 0 0 0
MFR kg 0 0 0 0 0 0 2.4E+02 0 0
MER kg 0 0 0 0 0 0 0 0 0
EEE MJ 0 0 9.37E+00 0 0 0 0 0 0
EET MJ 0 0 1.84E+01 0 0 0 0 0 0
4 Environmental Product Declaration - dormakaba - Security Revolving Door Geryon K9
HWD = Hazardous waste disposed; NHWD = Non-hazardous waste disposed; RWD = Radioactive waste disposed; CRU = Components for re-use;
MFR = Materials for recycling; MER = Materials for energy recovery; EEE = Exported electrical energy; EET = Exported thermal energy
RESULTS OF THE LCA – additional impact categories according to EN 15804+A2-optional:
1 piece SRD Geryon K9
Parameter Unit A1-A3 A4 A5 B6 C1 C2 C3 C4 D
Disease
PM 9.51E-05 2.02E-08 1.02E-08 1.32E-05 0 1E-08 1.58E-07 2.55E-07 -5.95E-05
incidence
IR kBq U235 eq 2.37E+02 8E-03 1.3E-02 3.11E+02 0 4E-03 1.08E-01 4.4E-02 -2.97E+02
ETP-fw CTUe 2.09E+04 3.86E+01 9.13E-01 5.35E+03 0 1.92E+01 1.21E+01 2.15E+01 -4.97E+03
HTP-c CTUh 4.7E-06 7.26E-10 5.72E-11 1.48E-07 0 3.6E-10 1.05E-09 3.19E-09 -2.24E-07
HTP-nc CTUh 3.02E-05 3.11E-08 3.81E-09 5.44E-06 0 1.54E-08 1.06E-07 3.51E-07 -7.74E-06
SQP SQP 2.59E+03 1.4E-01 5.74E-01 3.98E+03 0 6.9E-02 9.66E+00 7.85E+00 -4.15E+02
PM = Potential incidence of disease due to PM emissions; IR = Potential Human exposure efficiency relative to U235; ETP-fw = Potential comparative
Toxic Unit for ecosystems; HTP-c = Potential comparative Toxic Unit for humans (cancerogenic); HTP-nc = Potential comparative Toxic Unit for humans
(not cancerogenic); SQP = Potential soil quality index
Disclaimer 1 – for the indicator 'Potential Human exposure efficiency relative to U235'. This impact category deals mainly with the
eventual impact of low-dose ionizing radiation on human health of the nuclear fuel cycle. It does not consider effects due to possible
nuclear accidents, occupational exposure or radioactive waste disposal in underground facilities.
Potential ionizing radiation from the soil, radon and from some construction materials is also not measured by this indicator.
Disclaimer 2 – for the indicators 'abiotic depletion potential for non-fossil resources', 'abiotic depletion potential for fossil resources',
'water (user) deprivation potential, deprivation-weighted water consumption', 'potential comparative toxic unit for ecosystems', 'potential
comparative toxic unit for humans –
cancerogenic', 'Potential comparative toxic unit for humans - not cancerogenic', 'potential soil quality index'. The results of this
environmental impact indicator shall be used with care as the uncertainties on these results are high as there is limited experience with
the indicator.
This EPD was created using a software tool.
References
EN 16005 ISO 14025:2011-10, Environmental labels
EN 16005: 2013-01 and Amendment 2015-10 and declarations — Type III environmental declarations —
Power operated pedestrian door sets Principles and procedures.
EN 60335-2 2014/30/EU
EN 60335-2-103: 2016-05 Household and similar 2014/30/EU Electromagnetic Compatibility Directive OF THE
electrical appliances EUROPEAN PARLIAMENT AND OF THE COUNCIL of 26
February 2014 on the harmonization of the laws of the Member
EN 61000-3-2 States relating to electromagnetic compatibility.
EN 61000-3-2: 2015-03 Electromagnetic
compatibility (EMC) European Waste Catalogue (EWC)
COMMISSION DECISION of 18 December 2014
EN 61000-6-2 amending Decision 2000/532/EC on the list of waste
EN 61000-6-2: 2005 and Amendment:2011 pursuant to Directive 2008/98/EC of the European
Electromagnetic Compatibility (EMC) Parliament and of the Council
EN 61000-6-3 Machinery Directive 2006/42/EC
EN 61000-6-3: 2007 and A1:2011 Electromagnetic DIRECTIVE 2006/42/EC OF THE EUROPEAN
Compatibility (EMC) PARLIAMENT AND OF THE COUNCIL of 17 May
2006on machinery, and amending Directive 95/16/EC
ISO 12100
ISO 12100:2011-03 Safety of machinery REACH
Regulation (EC) No 1907/2006 of the European
ISO 13849- 1 Parliament and of the Council on the Registration,
ISO 13849-1: 2016-06 Safety of machinery Evaluation, Authorization and Restriction of Chemicals
(REACH)
ISO 13849- 2
ISO 13849-2: 2013-02 Safety of machinery ROHS Directive
Directive 2011/65/EU of the European Parliament and
EN 15804 of the Council of 8 June 2011 on the restriction of the
EN 15804+A2, Sustainability of construction works - use of certain hazardous substances in electrical and
Environmental Product Declarations - Core rules for the product electronic equipment
category of construction products.
Further References
ISO 9001
ISO 9001:2015-09 Quality management systems Requirements IBU 2021
General Instructions for the EPD programme of Institut Bauen
ISO 14025 und Umwelt e.V. Version 2.0, Berlin: Institut Bauen und Umwelt
5 Environmental Product Declaration - dormakaba - Security Revolving Door Geryon K9
e.V., 2021 LCA tool, ESC (Entrance System Control)
www.ibu-epd.com Tool No.: IBU-DOR-202109-LT1-EN
Developed by Sphera Solutions GmbH.
GaBi ts software
Sphera Solutions GmbH Gabi Software System and PCR Part A
Database for Life Cycle Engineering 19922020 PCR – Part A: Calculation Rules for the Life Cycle
Version 10.0.0.71 University of Stuttgart Assessment and Requirements on the Project Report
Leinfelden-Echterdingen according to EN 15804+A2:2019, Version 1.0, Institut
Bauen und Umwelt e.V., www.ibu-epd.com.
GaBi ts documentation
GaBi life cycle inventory data documentation PCR Part B
(https://www.gabisoftware.com/support/ PCR – Part B: Requirements on the EPD for electronic
gabi/gabidatabase[1]2020lcidocumentation/). and physical Access Control Systems, version 08/2021, Institut
Bauen und Umwelt e.V., www.ibu-epd.com.
LCA-tool dormakaba
6 Environmental Product Declaration - dormakaba - Security Revolving Door Geryon K9
Publisher
Institut Bauen und Umwelt e.V. +49 (0)30 3087748- 0
Hegelplatz 1 info@ibu-epd.com
10117 Berlin www.ibu-epd.com
Germany
Programme holder
Institut Bauen und Umwelt e.V. +49 (0)30 3087748- 0
Hegelplatz 1 info@ibu-epd.com
10117 Berlin www.ibu-epd.com
Germany
Author of the Life Cycle Assessment
dormakaba International Holding GmbH +49 2333 793-0
DORMA Platz 1 info.de@dormakaba.com
58256 Ennepetal www.dormakaba.com
Germany
Owner of the Declaration
dormakaba International Holding GmbH +49 2333 793-0
DORMA Platz 1 info.de@dormakaba.com
58256 Ennepetal www.dormakaba.com
Germany
7 Environmental Product Declaration - dormakaba - Security Revolving Door Geryon K9
