Environmental Product
Declaration
as per ISO 14025 and EN 15804
Owner of the declaration: Furhoffs Rostfria
Publisher: Kiwa-Ecobility Experts
Programme operator: Kiwa-Ecobility Experts
Registration number: EPD-Kiwa-EE-000343-EN
Issue date: 02.11.2023
Valid to: 02.11.2028
Furhoffs Rostfria AB
Stainless steel floor drains
Furo 142 (includes Furo 006, Furo
007, Furo 008, Furo 104, Furo 105,
Furo 139, Furo 141, Furo 170)
1. General information
AB Furhoffs Rostfria Stainless steel floor drains
Programme operator: Owner of the declaration:
Kiwa-Ecobility Experts AB FURHOFFS ROSTFRIA
Voltastr. 5 Haganders väg 2
13355 Berlin 541 34 Skövde
Germany Sweden
Registration number: Declared product / declared unit:
EPD-Kiwa-EE-000343-EN 1 piece of floor drain
This declaration is based on the Product Scope:
Category Rules: The EPD type: Cradle to gate with modules
PCR B for construction steel products (con- C1–C4 and module D.
struction steel products; draft; 2020-03-13) The floor drains are made of stainless steel.
Furhoffs productionsite is in Skövde.
Issue date: This specific EPD refers to a worst case prod-
02.11.2023 uct Furo 142 and includes Furo 006, Furo 007,
Furo 008, Furo 104, Furo 105, Furo 139, Furo
Valid to: 141 and Furo 170.
02.11.2028 Kiwa-Ecobility Experts assumes no liability for
manufacturer's information, LCA data and
evidence.
Verification:
The European standard EN 15804+A2:2019
serves as the core PCR.
Independent verification of the declaration
and data according to ISO 14025:2006.
☐internal ☒external
Frank Huppertz
(Head of Kiwa-Ecobility Experts)
Prof. Dr. Frank Heimbecher Elisabet Amat Guasch
(Chairman of the independent expert committee – (External verifier)
Kiwa-Ecobility Experts)
Page | 2 Furhoffs Rostfria — Furo 142
2. Product
2.1 Product description
All of the declared floor drains are produced of stainless steel. They are adjusted for being set in ce-
ment floors or wooden beam floors. The floor drains can be installed flexible in all different kinds of
flooring. They are applied at wet rooms in public baths and swimmingpools, kitchen and restaurants,
but also industrial buildings with varying exposure.
This EPD refers to a worst case product, which is Furo 142. It’s the worst case of a product group
consisting of Furo 006, Furo 007, Furo 008, Furo 104, Furo 105, Furo 139, Furo 141, Furo 170 and
Furo 142.
These products were grouped together since they are similar in material and application.
Table 1: Declared floor drains product group
Product group according to Furo 142 Weight (kg) Application
Stainless floor drain for wet areas in public
Ca. 2.3
spaces like shower and changing room
Furo 006
Stainless floor drain for wet areas in public
Ca. 2.4 spaces like swimming pool, shower and
changing room, wellness areas
Furo 007
Stainless floor drain for wet areas in
Ca. 4.5
public space
Furo 008
Stainless floor drain for kitchen, restaurant
Ca. 5,0
and industry with lower loads
Furo 104
Stainless floor drain for kitchen, restaurant
Ca. 8,6
and industry with lower loads
Furo 105
Stainless floor drain for areas with higher
Ca. 4.8 loads like industry, workshops, garage and
parking garage
Furo 139
Stainless floor drain for areas with higher
Ca. 5.7 loads like industry, workshops, garage and
parking garage
Furo 141
Stainless floor drain for high hygienic de-
Ca. 9.2
mands of the food industry
Furo 170
Stainless floor drain for areas with higher
Ca. 11.3 loads like industry, workshops, garage and
parking garage
Furo 142 (worst case)
Page | 3 Furhoffs Rostfria — Furo 142
2.2 Application
This product group Furo 142 consists of nine different types to cover several application possibilities.
2.3 Technical data
Furhoffs floor drains are available in different designs (models) and sizes. Weight and application
areas of the individual models can be found in table 1. The declared products have similarities since
they are made of the same materials. The main difference is weight/size and accessories, for example
grating. These differences are based on the fact, that there are floor drains for specific floor types,
applications, flow rates and loading classes.
Table 2: Characteristics of Furo 142
Characteristic (Furo142) Unit Value
EN 1.4404 Stainless Steel - -
SS-EN 1253-1, Flow rate, outlet side size 75 l/s 3,5
SS-EN 1253-1, Flow rate, outlet side size 110 l/s 3,7
SS-EN 1253-1, Flow rate, outlet bottom size 75 l/s 3,1
SS-EN 1253-1, Flow rate, outlet bottom size 110 l/s 4,0
SS-EN 1253-1, Loading class* - M125
*The loading class L15 refers to light traffic without forklifts, according to SS-EN 1253-1 with 10 kN load. The loading class M125 refers to
heavy traffic with lorrys and trucks, according to SS-EN 1253-1 with 85 kN load.
2.4 Placing on the market/ Application rules
The main markets are Sweden, Norway and to a less extent Finland.
The stainless steel floor drains are manufactured according to the requirements of the harmonized
standard SS-EN 1253-1:2015 Gullies for buildings - Part 1: Trapped floor gullies with a depth water
seal of at least 50 mm.
Furo 006, Furo 007, Furo 008, Furo 104, Furo 105 have type approvals.
2.5 Base materials / Ancillary materials
Table 3: Raw material for Furo 142
Raw material Furo 142 Unit Value
Base material
Stainless steel % 99,26%
EPDM rubber % 0,74%
Total base material kg 11,18
Ancillary material
Water % 64,43%
Cutting gas % 32,54%
Welding gas % 1,60%
Pickling liquid % 1,42%
Total ancillary material kg 12,01
Page | 4 Furhoffs Rostfria — Furo 142
2.6 Manufacturing
The manufacturing of the stainless steel floor drains contains the following processes:
• Delivery of raw materials
• Cutting
• Shaping
• Welding
• Pickling
• Blasting
• Assembling
• Packaging
odu e ec ared
ta ess stee odu e ot dec ared
u er
e o o
as cs
ard oard paper
ra sporta o a ufactur ra sport I sta a o se ra sporta o red ts a d
orr a d oads outs de
sse the s ste
ou dar
aste treat e t
a d
Figure 1: Graphic schematic process flow diagram for the Furhoffs production and module declared
2.7 Packaging
For delivery, the drains are wrapped into plastics, packed in cardboard boxes and transported on
europallets.
2.8 Reference Service Life (RSL)
The lifetime of stainless floor drains will be limited by the service life of the construction. The stain-
less steel products are specified for an intended service life of at least 50 years under the respective
loading classes / environmental conditions.
2.9 Other Information
For further information on this product please visit the webpage under the following link:
www.furhoffs.com
Page | 5 Furhoffs Rostfria — Furo 142
3. LCA: Calculation rules
3.1 Declared unit
One piece of floor drain is chosen as the declared unit.
Table 4: Declared unit and conversion factor for Furo 142
Product Furo 142 Unit Value
Declared Unit piece 1
Unit weight kg 11,18
Conversion factor to 1 0,089429
kg
piece
3.2 System boundary
This EPD was created in accordance with EN 15804 requirements and includes the production stage
and the End-of-life stage. According to EN 15804 this corresponds to product phases A1-A3, C1-C4
and D (EPD type "Cradle to gate, modules C1-C4 and module D" (A1-A3, C, D).
In a typical steel products manufacturing process, the individual components such as stainless steel
plates, welding consumables, pickling materials, and other ancillary materials are delivered to the
production facility. All the raw materials are mainly delivered by inland transport by truck. Until the
materials are actually used in production, they are stored in the warehouse.
All inputs, including raw materials, primary products, energy, and ancillary materials as well as the
accumulated waste are considered in the assessment. The use of the final product is not within the
manufacturer's sphere of influence. Therefore, modules B1-7 have not been considered.
Production stage
Module A1: This stage considers the extraction and processing of raw materials as well as energy
consumption. All installed raw materials of the products were analyzed, and the masses were deter-
mined. Steel material is given as a sum of different stainless steel raw materials.
Module A2: The raw materials are transported to the manufacturing plant. In this case, the model
includes relevant transportation of each raw material. Supplier information regarding the transport
distances and vehicle type were provided by Furhoffs Rostfria or chosen from relevant market pro-
files.
Module A3: This stage includes manufacturing of the products and packing. It also considers the en-
ergy consumption and waste generated at the manufacturing site. Energy and ancillary materials per
declared unit refer to an average share. Energy comes from non-fossile hydropower.
Module A4: not declared
Module A5: not declared
Modules B1 to B7: not declared. In normal use scenario, it is assumed that no maintenance (B2),
repair (B3), replacement (B4) and refurbishment (B5) is needed.
Module C1-C4: The modules C1 to C4 contain the end of life stage of the products: demoli-
tion/deconstruction, trans-port, waste processing and disposal.
Page | 6 Furhoffs Rostfria — Furo 142
Module D: Module D considers the reuse, recovery or recycling potential.
3.3 Estimates and assumptions
Energy and ancillary materials per declared unit refer to an average share of the Furhoffs yearly rev-
enue considering the declared floor drains.
3.4 Cut-off Criteria
All material flows that contribute to more than 1% of the total mass, energy or environmental impact
of the system have been considered in the LCA. It can be assumed that the neglected processes in
total contributed less than 5% to the considered impact categories.
The production of the machines, plants and other infrastructure required to produce the stainless
steel products were not taken into account in the LCA.
3.5 Period under review and Geographical reference area
All process-specific data was collected for the operating year 2022. The quantities of raw and auxilia-
ry materials as well as energy consumption have been recorded over the entire operating year 2022.
The geographical reference area is Sweden.
3.6 Data quality
Overall, the quality of the data can be considered as good. In the operating data survey all relevant
process-specific data could be collected. The data relating to the manufacturing phase of the stain-
less drains are determined by Furhoffs Rostfria and refers to the production site in Skövde.
Background data was taken from the Ecoinvent 3.6 database. The database is regularly checked and
thus complies with the requirements of ISO 14040/44 (background data not older than 10 years). The
background data meets the requirements of EN 15804. The quantities of raw materials, consumables
and supplies used as well as the energy consumption have been recorded and averaged over the
entire year of operation.
The general rule has been that specific data from specific production processes or average data de-
rived from specific processes must be given priority when calculating an EPD or Life Cycle Assess-
ment. Data for processes that the manufacturer cannot influence or choose, were backed up with
generic data.
3.7 Allocation
There are no co-products in the raw material supply phase, so no allocation methods were used at
this stage. There are no allocations during the manufacturing phase in the production facility.
3.8 Comparability
In principle, a comparison or assessment of the environmental impacts of different products is only
possible if they have been prepared in accordance with EN 15804. For the evaluation of the
comparability, the following aspects have to be considered in particular: PCR used , functional or
declared unit, geographical reference, definition of the system boundary, declared modules, data
Page | 7 Furhoffs Rostfria — Furo 142
selection (primary or secondary data, background database, data quality), scenarios used for use and
disposal phases, and the life cycle inventory (data collection, calculation methods, allocations,
validity period). PCRs and general program instructions of different EPDs programs may differ. A
comparability needs to be evaluated. For further guidance see EN 15804+A2 (5.3 Comparability of
EPD for construction products) and ISO 14025 (6.7.2 Requirements for comparability).
4. LCA: Scenarios and additional technical information
Module A3:
Use of water is declared only for technological process (pickling); no waste scenario is assumed as no
wastewater occurs. For the p ck qu d there’s ee a waste scenario assumed. The generated
production waste concerning the ancillary material is stated per declared unit. For raw material only
certain inputs cause production waste. These inputs are declared in kg.
Module C1-C4:
The floor drains are assumed to be disposed of in Northern Europe. The floor drains are assumed to
be dismantled using hand tools (C1) and transported 50 km to a local recycling (C2).
The product is disposed according to the selected waste scenario: recovery of materials, recycling
94%, reuse 5 % (C3). The fluff sorted from the shredded metal is landfill by 1% (C4).
Module D:
The recycled metals are credited an avoided production of primary steel.
5. LCA: Results
The following tables show the results of the impact assessment indicators, resource use, waste and
other output streams. The results presented here refer to the declared average product.
Disclaimer on ADP-e, ADP-f, WDP, ETP-fw, HTP-c, HTP-nc, SQP: The results of these environmental
impact indicators must be used with caution, as the uncertainties in these results are high or as there
is limited experience with the indicator.
Disclaimer on IR: This impact category mainly addresses the potential effect of low dose ionizing ra-
diation on human health in the nuclear fuel cycle. It does not consider effects due to possible nuclear
accidents and occupational exposures, nor does it consider radioactive waste disposal in under-
ground facilities. Potential ionizing radiation from soil, radon, and some building materials is also not
measured by this indicator.
Page | 8 Furhoffs Rostfria — Furo 142
Description of the system boundary
Construction process Benefits and loads beyond
Product stage Use stage End of life stage
stage the system boundaries
la ir e wt a am Ry lp p u s t r o p s n a r T u n a M-g n ir u t c a f t r o p s n a r Tu n a m m o r-
f
o t r e r u t c a fe s u fo e c a lp n o it c u r ts n o
C
n o it a lla ts n -is s e c o r p e s U n ia M-e c n a n e t r ia p e R tn e m e c a lp e
R
r u fe R-n e m h s ib la n o it a r e p Oe s u y g r e n e la n o it a r e p Oe s u r e t a w e D- n o it c u r ts n o cn o itilo m e d
/
t r o p s n a r T e ts a Wg n is s e c o r p la s o p s iD e s u e R-y r e v o c e R- g n ilc y c e R- a itn e t o pl
A1 A2 A3 A4 A5 B1 B2 B3 B4 B5 B6 B7 C1 C2 C3 C4 D
X X X MND MND MND MND MND MND MND MND MND X X X X X
X=Module declared | MND=Module not declared
LCA results - Indicators describing environmental impacts based on the impact assessment (LCIA): 1 piece Furo142 (EN 15804+A2)
Page | 9 Furhoffs Rostfria — Furo 142
Parameter Unit A1 A2 A3 C1 C2 C3 C4 D
Core environmental impact indicators (EN 15804+A2)
GWP-total kg CO2 eqv. 5,64E+01 7,20E-01 8,68E+00 0,00E+00 7,35E-02 4,48E-01 3,05E-03 -1,36E+01
GWP-f kg CO2 eqv. 5,60E+01 7,20E-01 1,23E+01 0,00E+00 7,35E-02 4,48E-01 3,05E-03 -1,38E+01
GWP-b kg CO2 eqv. 4,39E-01 3,84E-04 -3,63E+00 0,00E+00 3,39E-05 2,33E-05 3,06E-06 1,40E-01
GWP-luluc kg CO2 eqv. 4,11E-02 2,52E-04 2,05E-02 0,00E+00 2,69E-05 3,76E-06 2,50E-07 9,39E-03
ODP kg CFC 11 eqv. 3,04E-06 1,64E-07 8,00E-07 0,00E+00 1,62E-08 1,18E-09 2,95E-10 -3,55E-07
AP mol H+ eqv. 3,60E-01 2,94E-03 7,89E-02 0,00E+00 4,26E-04 7,41E-05 7,08E-06 -5,39E-02
EP-fw kg P eqv. 2,38E-03 5,65E-06 5,22E-04 0,00E+00 7,41E-07 1,45E-07 9,71E-09 -4,96E-04
EP-m kg N eqv. 6,04E-02 8,73E-04 1,41E-02 0,00E+00 1,50E-04 2,70E-05 2,84E-06 -9,96E-03
EP-T mol N eqv. 6,92E-01 9,65E-03 1,58E-01 0,00E+00 1,66E-03 2,99E-04 2,67E-05 -1,16E-01
POCP kg NMVOC eqv. 2,19E-01 2,95E-03 4,11E-02 0,00E+00 4,73E-04 7,54E-05 8,27E-06 -7,80E-02
ADP-mm kg Sb-eqv. 2,05E-03 1,95E-05 4,41E-04 0,00E+00 1,86E-06 1,05E-07 7,23E-09 -9,05E-06
ADP-f MJ 6,27E+02 1,09E+01 1,53E+02 0,00E+00 1,11E+00 9,24E-02 2,05E-02 -9,91E+01
WDP m3 world eqv. 1,05E+01 3,02E-02 3,80E+00 0,00E+00 3,96E-03 5,81E-03 9,11E-04 -2,54E+00
Additional environmental impact indicators (EN 15804+A2)
PM disease incidence 4,76E-06 5,02E-08 1,03E-06 0,00E+00 6,61E-09 4,70E-10 1,37E-10 -8,20E-07
IR kBq U235 eqv. 1,78E+00 4,74E-02 5,44E-01 0,00E+00 4,64E-03 2,58E-04 8,33E-05 2,12E-01
ETP-fw CTUe 1,95E+03 8,69E+00 3,76E+02 0,00E+00 9,88E-01 7,64E-01 1,50E-02 -4,60E+02
HTP-c CTUh 8,84E-07 2,44E-10 1,83E-07 0,00E+00 3,20E-11 7,86E-12 3,61E-13 -6,22E-09
HTP-nc CTUh 2,54E-06 9,48E-09 1,11E-06 0,00E+00 1,08E-09 3,51E-10 1,04E-11 2,47E-06
SQP Pt 3,12E+02 7,48E+00 4,84E+02 0,00E+00 9,61E-01 4,85E-02 4,41E-02 -2,17E+01
ADP-mm= Abiotic depletion potential for non-fossil resources | ADP-f=Abiotic depletion for fossil resources potential | AP= Acidification potential, Accumulated Exceedance | EP-fw = Eutrophication potential, fraction of nutrients reaching
freshwater end compartment | EP-m= Eutrophication potential, fraction of nutrients reaching marine end compartment| EP-T= Eutrophication potential, Accumulated Exceedance | GWP-b=Global Warming Potential biogenic | GWP-
f=Global Warming Potential fossil fuels | GWP-luluc=Global Warming Potential land use and land use change |GWP-total=Global Warming Potential total| ODP=Depletion potential of the stratospheric ozone layer |POCP=Formation poten-
tial of tropospheric ozone | WDP=Water (user) deprivation potential, deprivation- weighted water consumption | ETP-fw=Potential Comparative Toxic Unit for ecosystems | HTP-c=Potential Toxic Unit for Humans toxicity, cancer | HTP-nc=
Potential Toxic Unit for humans, non-cancer | IRP=Potential Human exposure efficiency relative to U235, human health | PM=Potential incidence of disease due to Particulate Matter emissions | SQP=Potential soil quality index
Page | 10 Furhoffs Rostfria — Furo 142
LCA results - Indicators describing resource use and environmental information derived from life cycle inventory (LCI): 1 piece Furo142 (EN 15804+A2)
Parameter Unit A1 A2 A3 C1 C2 C3 C4 D
PERE MJ 1,57E+02 1,53E-01 1,29E+02 0,00E+00 1,39E-02 4,57E-03 2,06E-04 2,45E+00
PERM MJ 0,00E+00 0,00E+00 3,19E+01 0,00E+00 0,00E+00 0,00E+00 0,00E+00 0,00E+00
PERT MJ 1,57E+02 1,53E-01 1,61E+02 0,00E+00 1,39E-02 4,57E-03 2,06E-04 2,45E+00
PENRE MJ 6,67E+02 1,15E+01 1,62E+02 0,00E+00 1,18E+00 9,94E-02 2,18E-02 -1,03E+02
PENRM MJ 0,00E+00 0,00E+00 1,48E+00 0,00E+00 0,00E+00 0,00E+00 0,00E+00 -2,36E-01
PENRT MJ 6,67E+02 1,15E+01 1,63E+02 0,00E+00 1,18E+00 9,94E-02 2,18E-02 -1,03E+02
SM Kg 1,44E+00 0,00E+00 3,12E-01 0,00E+00 0,00E+00 0,00E+00 0,00E+00 0,00E+00
RSF MJ 0,00E+00 0,00E+00 0,00E+00 0,00E+00 0,00E+00 0,00E+00 0,00E+00 0,00E+00
NRSF MJ 0,00E+00 0,00E+00 0,00E+00 0,00E+00 0,00E+00 0,00E+00 0,00E+00 0,00E+00
FW M3 3,47E-01 1,14E-03 1,17E-01 0,00E+00 1,35E-04 5,90E-04 2,18E-05 -4,86E-02
HWD Kg 1,19E-03 2,84E-05 -4,92E-05 0,00E+00 2,81E-06 4,15E-07 3,07E-08 -1,63E-03
NHWD Kg 6,34E+01 5,19E-01 1,36E+01 0,00E+00 7,03E-02 1,19E-02 1,28E-01 -1,30E+00
RWD Kg 1,64E-03 7,40E-05 4,74E-04 0,00E+00 7,28E-06 3,20E-07 1,32E-07 6,55E-05
CRU Kg 0,00E+00 0,00E+00 1,20E-01 0,00E+00 0,00E+00 5,55E-01 0,00E+00 0,00E+00
MFR Kg 0,00E+00 0,00E+00 2,26E+00 0,00E+00 0,00E+00 1,04E+01 0,00E+00 0,00E+00
MER Kg 0,00E+00 0,00E+00 0,00E+00 0,00E+00 0,00E+00 0,00E+00 0,00E+00 0,00E+00
EET MJ 0,00E+00 0,00E+00 0,00E+00 0,00E+00 0,00E+00 0,00E+00 0,00E+00 0,00E+00
EEE MJ 0,00E+00 0,00E+00 0,00E+00 0,00E+00 0,00E+00 0,00E+00 0,00E+00 0,00E+00
PERE=Use of renewable primary energy excluding renewable primary energy resources used as raw materials | PERM= Use of renewable primary energy resources used as raw materials | PERT=Total use of renewable primary energy
resources | PENRE= Use of non-renewable primary energy excluding non-renewable primary energy resources used as raw materials | PENRM= Use of non-renewable primary energy resources used as raw materials | PENRT= Total use of
non-renewable primary energy resources | SM=Use of secondary material | RSF=Use of renewable secondary fuels | NRSF=Use of non-renewable secondary fuels | FW=Use of fresh water | HWD=Hazardous waste disposed | NHWD=Non-
hazardous waste disposed | RWD=Radioactive waste disposed | CRU=Components for re-use | MFR=Materials for recycling | MER=Materials for energy recovery | EET=Exported energy, thermical | EE=Exported energy, electrical
LCA results - information on biogenic carbon content at the factory gate: 1 piece Furo142 (EN 15804+A2)
Parameter Unit Value
biogenic carbon content in product kg C 0
biogenic carbon content in accompanying packaging kg C 1,021
NOTE 1 piece biogenic carbon is equivalent to 44/12 kg CO2
Page | 11 Furhoffs Rostfria — Furo 142
6. LCA: Interpretation
6.1 Dominance analysis
The results show that the production of stainless steel (A1) is the dominating process in most of the
environmental impact categories. Additionally, the steel has the largest contribution in the corre-
sponding avoided production of materials beyond the system boundary (D). This stems especially
from the steel content that is costly to produce, but which can be recycled at the end-of-life. The
packaging materials (pallets and cardboard) contribute to a biogenic CO2 uptake. The majority of the
CO2 emissions within the impact category GWP-biogenic originate from the packaging. Since the
module A5 which includes the waste processing of packaging is not declared there seems to be a
disbalance of biogenic CO2 emissions. Therefore, the alleged disbalance can be explained by the fact
that the module A5 is not included in the EPD declaration.
The electrical energy for the production comes from non-fossil hydropower and causes low impact.
Furo142
100%
80%
60%
40%
20%
0%
-20%
-40%
-60%
-80%
-100%
A1 A2 A3 C1 C2 C3 C4 D
Figure 2: Influence of the modules A1 – A3, C1 - C4 and D on the environmental core indicators for
Furo 142
6.3 Data quality
The background data is taken from Ecoinvent database version 3.6 (2019). The life cycle assessment
was modeled with the NIBE tool. Geographical reference space of the background data is global or
Europe. Almost all consistent datasets contained in the Ecoinvent database are documented and can
be viewed in the online Ecoinvent documentation.
Overall, the quality of the data can be considered as good. In the operating data survey all relevant
process-specific data could be collected. The data relating to the manufacturing phase of the stain-
less steel floor drains are determined by Furhoffs Rostfria and refers to the production site in Skövde,
Sweden.
Page | 12 Furhoffs Rostfria — Furo 142
The general rule has been that specific data from specific production processes or average data de-
rived from specific processes must be given priority when calculating an EPD or Life Cycle Assess-
ment. Data for processes that the manufacturer cannot influence or choose, were backed up with
generic data.
7. References
Ecoinvent 2019 Ecoinvent Datenbank Version 3.6 (2019)
EN 15804 EN 15804:2012+A2:2019: Sustainability of construction works — Environ-
mental Product Declarations — Core rules for the product category of con-
struction products
ISO 14025 ISO 14025:2006 Environmental labels and declarations — Type III environ-
mental declarations — Principles and procedures EN 13249
ISO 14040 ISO 14040:2006 Environmental management - Life cycle assessment - Princi-
ples and framework
ISO 14044 ISO 14044:2006 Environmental management - Life cycle assessment - Re-
quirements and guidelines
NMD 2019 NMD STICHTING NATIONAL ENVIRONMENTAL DATABASE: Environmental
Performance Assessment Method for Construction; 1.1 (March 2022); Rijs-
wijk
PCR A Kiwa-Ecobility Experts, Berlin, 2022: PCR A – General Program Category Rules
for Construction Products from the EPD programme of Kiwa-Ecobility Ex-
perts; Version 2.1
PCR B Kiwa-Ecobility Experts, Berlin, 2020: PCR B – Product Category Rules for steel
construction products, Requirements on the Environmental Product Declara-
tions for steel construction products; Version 2020-03-13 (draft)
R<THiNK 2023 R<THiNK; Online-EPD-Tool by NIBE B.V.
SimaPro Software Industry data LCA library; website: https://simapro.com/databases/industry-
data-lca-library/
Page | 13 Furhoffs Rostfria — Furo 142
Publisher Mail DE.Ecobility.Experts@kiwa.c
Kiwa-Ecobility Experts om
Voltastr.5 Web https://www.kiwa.com/de/
13355 Berlin de/themes/ecobility-
Germany experts/ecobility-experts/
Programme operator Mail DE.Ecobility.Experts@kiwa.c
Kiwa-Ecobility Experts om
Voltastr. 5 Web https://www.kiwa.com/de/
13355 Berlin de/themes/ecobility-
Germany experts/ecobility-experts/
LCA Practitioner Tel. +46-10 479 30 00
Kiwa Certification AB Mail Se.Bygg@kiwa.com
Campus Gräsvik 1 Web https://www.kiwa.se
37175 Karlskrona
Sweden
Owner of the declaration Tel. 0500 44 45 46
AB FURHOFFS ROSTFRIA Mail info@furhoffs.se
Haganders väg 2 Web https://www.furhoffs.com
541 34 Skövde
Sweden
Kiwa-Ecobility Experts -
established member of
Page | 14 Furhoffs Rostfria — Furo 142
