ENVIRONMENTAL PRODUCT DECLARATION
as per ISO 14025 and EN 15804+A2
Owner of the Declaration WILSONART
Publisher Institut Bauen und Umwelt e.V. (IBU)
Programme holder Institut Bauen und Umwelt e.V. (IBU)
Declaration number EPD-WIL-20230465-CBA1-EN
Issue date 25/10/2023
Valid to 03/10/2028
Wall Panelling System
Wilsonart
www.ibu-epd.com | https://epd-online.com
1. General Information
Wilsonart Wall Panelling System
Programme holder Owner of the declaration
IBU – Institut Bauen und Umwelt e.V. WILSONART
Hegelplatz 1 Rixon Road 9-29
10117 Berlin NN8 4B Wellingborough, Northamptonshire
Germany United Kingdom
Declaration number Declared product / declared unit
EPD-WIL-20230465-CBA1-EN 1 square meter of wall panel
This declaration is based on the product category rules: Scope:
Decorative board for interior use, 01/08/2021 The declaration covers a tongue-and-groove system of bathroom and
(PCR checked and approved by the SVR) wetroom wall panels thickness 11,7 mm+/-0,6 mm. The system is named
bathroom and wetroom wall panel. The declaration covers the total range
of colors. The product is manufactured by WILSONART in its
Issue date Wellingborough plant (UK).
The owner of the declaration shall be liable for the underlying information
25/10/2023
and evidence; the IBU shall not be liable with respect to manufacturer
information, life cycle assessment data and evidences.
Valid to
The EPD was created according to the specifications of EN 15804+A2. In
03/10/2028 the following, the standard will be simplified as EN 15804.
Verification
The standard EN 15804 serves as the core PCR
Independent verification of the declaration and data according to ISO
14025:2011
internally X externally
Dipl.-Ing. Hans Peters
(Chairman of Institut Bauen und Umwelt e.V.)
Florian Pronold Dr Naeem Adibi,
(Managing Director Institut Bauen und Umwelt e.V.) (Independent verifier)
1 Environmental Product Declaration - Wilsonart - Wall Panelling System
2. Product
according to EN438-7:2005 (High-pressure decorative
2.1 Product description/Product definition laminates (HPL) - Sheets based on thermosetting resins
Wall panelling system described in the EPD are made from a (Usually called Laminates) - Part 7: Compact laminate and HPL
water-resistant composite material board, glued on 2 sides with composite panels for internal and external wall and ceiling
High Pressure Laminate (HPL), conforming to EN438-3 with a finishes)
humid-resistant glue. The complete panel conforms to EN438-
7. The decorative side, made with HPL, permits a large range 2.4 Delivery status
of decors and finishes. The backing side is made with a Standard size of panels are:
balancing HPL. 242 × 120 cm rounded edge / tongue
A wall panel has a rounded edge for optimum finish and 242 × 120 cm tongue / groove
hygiene. The tongue-and-groove assembly system permits 242 × 60 cm tongue / groove
ease of installation and seamless joints. 242 × 58 cm rounded edge / rounded edge
The final installation is made with Complete adhesive and 242 × 16 cm rounded edge / tongue
Complete colour-matched sealants, ensuring long-term Thickness 11,7 mm +/- 0,6 mm
prevention of any water ingress. For the placing on the market
in the European Union/European Free Trade Association 2.5 Base materials/Ancillary materials
(EU/EFTA) (except for Switzerland) the Regulation (EU) No The composition of the wall panels in mass is:
305/211 applies. The products need a Declaration of . 73 % water-resistant composite board
Performance taking into consideration EN 438-7, and all have a . 26 % HPL surface and backing
CE-marking. . 1 % PUR glue.
2.2 Application The product contains 14 % recycled content from HPL (paper)
The wall panel system is a patented wall-covering solution and board (PVC) (pre-consumer and post-consumer).
suitable for new or refurbished bathrooms and wetrooms. It can The core is a water-resistant composite board density of 600
be used instead of or on top of existing tiling without having to kg/m3.
smooth the surface down first, or on moisture resistant The surface and back side are HPL conforming to EN438-3.
plasterboard. The gluing is made with water-resistant PUR glue.
2.3 Technical Data The product contains other carcinogenic, mutagenic, reprotoxic
Wall panels are evaluated according EN438-2 as HPL bonded (CMR) substances of category 1A or 1B that are not on the
board. Detailed information can be found in the technical data candidate list, above 0.1 by weight % in at least one sub-
sheet. product: no.
Constructional data
Biocidal products have been added to this building product or it
Name Value Unit
has been treated with biocidal products (this refers to treated
Gross density 700 kg/m3 goods within the meaning of the Biocidal Products Regulation
Grammage 8.34 kg/m2 (EU) No. 528/2012): yes.
Impact resistance acc. to EN It contains a biocide whose active ingredient is silver phosphate
438-2-21 600 mm glass which complies with the REACH and European Biocidal
Products regulations (EU) No. 528/2012.
Resistance to scratches acc. Min D3 except BRI
Degree
to EN 438-2-25 min D2 2.6 Manufacture
Light resistance acc. to EN 4 - 5 - 1. PUR calendar press: gluing of HPL on 2 sides on water-
438-2-27 resistant composite board with PUR water-resistant glue
Surface adhesion ISO 2. Postforming of HPL for panels with round edge
1 MPa
13894-1-9 3. Profiling Tongue and groove and edge
Durability - resistance in wet 4. Unit packaging
conditions - 48 h at 40°C EN Mass increase < 8 % The Quality management system is certified: ISO 9001.
438-2-15 modified
2.7 Environment and health during manufacturing
Durability - resistance in wet
The production conditions do not demand any special health
conditions 48h at 40°C EN >= 4 Degree
protection measures over and beyond the legal requirements.
438-2-15 modified
Air: the constitutional valid regulations are observed. The
mm/linear
Flatness EN 438-2-9 <= 3 emissions into the air are below the legally required thresholds.
meter
Water: The process doesn't use or reject water.
Height: =/- 1,5 - Soil: There is no impact on soil.
Dimensional tolerance EN
Width: +/- 1 - mm The Environmental management system is certified: ISO
438-2-5 and 6
Thickness: +0,4/-0,2 14001.
mm/linear
Squareness EN 438-2-8 <=1,5 2.8 Product processing/Installation
meter
Wall panels can be cut using woodworking tools with carbide-
Stain resistance EN 438-2- Group 1&2: 5 -
Grade tipped blades and bits.
26 Group 3: 4
Follow all the usual health and safety precautions when
Resistance to abrasion EN Taber
150-450 processing these panels about weight, dust and sharp edges.
438-2-10 rounds
Use appropriate personal protective equipment.
Performance values of the product are stated in the declaration The dust produced by processing technical panelling solutions
of performance, in relation to its essential characteristics may irritate the skin or lungs, so use a dust collector whenever
2 Environmental Product Declaration - Wilsonart - Wall Panelling System
cutting wood and wear appropriate personal protective The estimated service life of wall panels depends on the area
equipment. of application (private or commercial use), the users
The assembly of the panels is done by gluing with Complete themselves and the maintenance of the product. According to
adhesive. the Federal Office for Building and Regional Planning (BBSR) a
For renovation, the panels can be bonded directly on tiling. reference service life of 20 years can be assumed for
The correct preparation of the substrate (flatness, laminate/plastic coverings. The use stage (module B2) is
waterproofing...) is key and detailed in the processing brochure. declared in this EPD for 20 years of usage assuming 50 %
The assembly is done thanks to the tongue and groove system domestic and 50 % commercial level of use.
and the coloured connection joint Complete provides a
seamless joint. 2.13 Extraordinary effects
Detailed information and processing are available at Fire
www.bushboard.co.uk. Wall panels are classified as E according to EN13501-1 and M3
according to NFP 92-501.
2.9 Packaging Water
Wall panels are delivered unit-packed, and edge-protected The wall panel system is designed for use in an interior fitting of
using cardboard. bathrooms or wetroom walls.
Cardboard can be recycled materially or energetically. When installed according to the technical guideline and using
Pallets are used for the delivery. The pallets can be reused. Complete adhesives and sealants, the water doesn't have any
impact on the the wall panel system.
2.10 Condition of use No substances that can be hazardous to water are washed out.
The composition during the use phase refers to the composition
during the manufacturing. Mechanical destruction
Core and HPL panels are chemically inert and the bonding The surface of HPL of wall panel system gives good
agents are chemically stable and permanently bonded to the performance regarding impact, according to EN 438-3
core. specification. The application of wall panel system is a vertical
application for wall panelling in bathrooms and wetrooms
2.11 Environment and health during use
therefore not subject to strong mechanical aggression.
Environmental protection: Moreover in case of severe damage the damaged panels
When the described products are used properly in accordance should be replaced.
with the area of application, there is no risk of water, air, or No hazardous substances are released during mechanical
ground contamination according to the current state of destruction.
knowledge.
2.14 Re-use phase
Health protection: Currently, there is no possible re-use or recycling option. The
When used normally and in accordance with the intended scenario for the end of life is a landfill.
purpose, no health risks or restrictions are to be anticipated
with wall panels. 2.15 Disposal
Except for minor amounts of formaldehyde in quantities that are Waste from wall panels is classed according to the European
harmless to health, no emissions of hazardous substances can Waste Catalogue under the six-digit waste code 20 03 01. It is
be detected. defined as «mixed municipal waste» which can be disposed of
VOC emissions are measured for A ratings in tests on walls as household or commercial waste.
with a loading factor of 1.0 m2/m3.
This is in line with the current state of knowledge. 2.16 Further information
Detailed information and recommendations are available on
2.12 Reference service life www.bushboard.co.uk.
3. LCA: Calculation rules
Modules A1-A3 also include the manufacturing and
3.1 Declared Unit supply of energy.
This declaration refers to the declared unit of 1 m² of wall panel. • The scenario for the transport of the product to the
The weight of the product is 8.34 kg/m². construction site is declared in module A4.
Declared unit and mass reference • The treatment of packaging materials at installation,
installation auxiliaries as well as installation losses are
Name Value Unit
declared in module A5.
Declared unit 1 m2 • The use stage includes emissions occurring during the
Grammage 8.34 kg/m2 lifetime of the product (B1) as well as the maintenance
Layer thickness 0.0117 m stage/cleaning (B2).
• Two end-of-life scenarios are declared in the EPD. They
include manual dismantling (C1), transportation to waste
processing (C2),
3.2 System boundary
• Scenario 1: 100 % thermal treatment with energy
The type of EPD is cradle to gate with options. The additional
recovery (C3/1). Credits for electricity and thermal
modules are modules A4, A5, B1 and B2.
energy, which result from energy recovery in modules
A5 and C3, are declared in module D/1.
Considered product stages:
• Scenario 2: 100 % landfilling (C4/2). Credits for
• Production of pre-products, extraction of energy electricity and thermal energy, which result from energy
carriers, raw material transportation, manufacture of recovery in module A5, are declared in module D/2.
product and packaging materials are declared in • The CO incorporation in the product (from the
2
modules A1-A3.
sequestration in the paper material) is
3 Environmental Product Declaration - Wilsonart - Wall Panelling System
considered. The C-balance is closed by considering the • All primary and secondary data are modelled
biotic CO emissions according to the incorporation on to be specific to the technologies or
2
the input side. technology mixes under study. Where
technology-specific data is unavailable,
3.3 Estimates and assumptions proxy data are used. The overall
The following assumptions are included in the EPD: technological representativeness is
considered to be good.
• It is assumed that packaging materials are disposed of
• Primary data are collected by the client using
via incineration (wooden pallets) and recycling
a specifically adapted spreadsheet. Sphera
(cardboard).
supported the data collection by preparing a
• Distance to the end of life of non-hazardous waste is
specific questionnaire and virtual or onsite
assumed as 50km.
support.
3.4 Cut-off criteria Overall, the data quality can be described as good.
The packaging of the raw materials, as well as their disposal, is The primary data collection has been done thoroughly;
not considered in the scope of this study. all relevant flows are considered.
Transportation of installation auxiliaries' materials is also not
3.7 Period under review
considered in the scope of this study.
The period under review for the collection of production data is
3.5 Background data the year 2021.
The background data has been taken from the latest
3.8 Geographic Representativeness
available GaBi database CUP 2022.1. The requirements for
Land or region, in which the declared product system is
data quality and background data correspond to the
manufactured, used or handled at the end of the product´s
specifications of the PCR Part A.
lifespan: Europe
3.6 Data quality
The requirements on the data quality and the
3.9 Allocation
background data correspond to the provisions in EN 15804 and
The production process does not deliver any co-products. The
the IBU PCR part A (IBU 2020) respectively:
applied software model does not contain any allocation.
• All primary data are collected for the year The overall production of Wilsonart comprises further products
2021. All secondary data come from the GaBi besides the products considered in this study. Data for electrical
databases and are representative of the years energy refers to the declared product. During data collection,
2017-2022. As the study intended to compare the the allocation is done via quantities (mass) produced.
product systems for the reference year
2021, temporal representativeness is good. 3.10 Comparability
• All primary and secondary data are collected Basically, a comparison or an evaluation of EPD data is only
specific to the countries/regions under study. possible if all the data sets to be compared were created
Where country/region-specific data are according to EN 15804 and the building context, respectively
unavailable, proxy data are used. The overall the product-specific characteristics of performance, are taken
geographical representativeness is into account. Background dataset: GaBi ts software, CUP
considered to be good. 2022.1.
4. LCA: Scenarios and additional technical information
Name Value Unit
Characteristic product properties of biogenic carbon
Litres of fuel (truck Euro 6) 0.013 l/100km
Biogenic carbon is present in the product and the packaging
Transport distance 600 km
materials.
Capacity utilisation (including empty runs) 61 %
Note: 1 kg biogenic Carbon is equivalent to 44/12 kg of CO
2 Installation into the building (A5)
Information on describing the biogenic Carbon Content at The installation of the wall panelling system board is done
factory gate manually with some electric tools (e.g. cutting saw). Adhesive
Name ValueUnit and sealant are needed for the installation.
kg
Biogenic carbon content in product 0.66 C Installation losses have been accounted for in module A5.
Product losses have been considered as 15 %. Losses are
Biogenic carbon content in accompanying kg
0.66 disposed of in a landfill.
packaging C
The packaging material treatment and disposal are also
considered in module A5.
The following technical information is a basis for the declared
Name ValueUnit
modules.
Auxiliary (adhesive and sealant) 0.18 kg
Transport to the building site (A4)
Electricity consumption (for cutting) 0.06 kWh
Module A4 considers a 600 km truck transport from the
Material loss (15 %) 1.25 kg
manufacturing plant in the UK to an average European
Output substances following waste treatment on
customer site. 1.605 kg
site (packaging materials)
Packaging material:
Cardboard: 0,105 kg/m²
4 Environmental Product Declaration - Wilsonart - Wall Panelling System
Wood pallets: 1,5 kg/m²
Reference service life
Name Value Unit
Use (B1)
Life Span according to the manufacturer 20 a
Emissions to air occur during the use stage of the product. The
following emissions are considered in module B1. End of life (C1-C4)
Name Value Unit The deconstruction (module C1) is assumed to be done
Formaldehyde emissions (for the RSL) 1,60E-08 kg/m² manually (no environmental impact).
VOC emissions (for the RSL) 7,5E-09 kg/m²
The transport to waste processing (module C2) is assumed to
Maintenance (B2) be 50 km.
Module B2 includes the cleaning of the board. Water and
Scenario 1 : Thermal treatment with energy recovery (C3/1)
detergent are required for the cleaning. The scenario considers
Scenario 2 : Landfilling (C4/2)
installation in the following conditions: 50 % residential (1
cleaning/week) and 50 % hotel (1 cleaning/day - 70 % load). Name Value Unit
This results in 154 cleanings per year. The following table Collected as mixed construction waste 8.34 kg
documents the water and auxiliaries consumption for the
Landfilling (Scenario 1) 8.34 kg
cleaning of 1 m² per year.
Energy recovery (Scenario 2) 8.34 kg
Name Value Unit
Water consumption 0.0077 m3
Reuse, recovery and/or recycling potentials (D)
Auxiliary (detergent) 0.123 kg Module D/1 includes the potential benefits in form of energy
The estimated service life of wall panelling system depends on recovery of the incineration process in A5 (incineration of
the area of application (private or commercial use), the users packaging wastes) and C4 (combustion of the product).
themselves and the maintenance of the product. According to
BBSR a reference service life of 20 years can be assumed for Module D/2 includes the potential benefits in form of energy
laminate/plastic coverings. The use stage (module B2) is recovery of the incineration process in A5 (incineration of
declared in this EPD for 20 years of usage assuming 50 % packaging wastes).
domestic and 50 % commercial level of use.
5 Environmental Product Declaration - Wilsonart - Wall Panelling System
5. LCA: Results
The following tables display the environmentally relevant results according to EN 15804+A2 for 1 m² Wall Panelling System.
Two end-of-life scenarios are declared in the EPD:
C3/1: 100 % thermal treatment of the product with energy recovery
D/1: benefits in form of energy recovery of the incineration process in A5 (incineration of packaging wastes) and C4 (combustion of the
product).
C4/2: 100 % landfilling
D/2: benefits in form of energy recovery of the incineration process in A5 (incineration of packaging wastes).
DESCRIPTION OF THE SYSTEM BOUNDARY (X = INCLUDED IN LCA; ND = MODULE OR INDICATOR NOT DECLARED; MNR =
MODULE NOT RELEVANT)
Benefits and
Construction loads beyond
Product stage Use stage End of life stage
process stage the system
boundaries
la ire ta m w a Ry lp p u s tro p s n a rT g n iru tc a fu n a M e h t m o rf tro p s n a rTe tis e h t o t e ta g y lb m e s s A e s U e c n a n e tn ia M ria p e R tn e m e c a lp e R tn e m h s ib ru fe R y g re n e la n o ita re p Oe s u re ta w la n o ita re p Oe s u n o itc u rts n o c -e Dn o itilo m e d tro p s n a rT g n is s e c o rp e ts a W la s o p s iD -e s u e R-y re v o c e R-g n ilc y c e Rla itn e to p
A1 A2 A3 A4 A5 B1 B2 B3 B4 B5 B6 B7 C1 C2 C3 C4 D
X X X X X X X MNR MNR MNR MND MND X X X X X
RESULTS OF THE LCA - ENVIRONMENTAL IMPACT according to EN 15804+A2: 1 m² Wall Panelling System
Parameter Unit A1-A3 A4 A5 B1 B2 C1 C2 C3/1 C3/2 C4/1 C4/2 D/1 D/2
GWP-total kg CO 2 eq 4.3E+01 4.55E-01 1.23E+01 0 1.96E+00 0 3.25E-02 1.84E+01 0 0 5.39E+00 -5.02E+00 -9.51E-01
GWP-fossil kg CO 2 eq 4.77E+01 4.5E-01 1.02E+01 0 1.87E+00 0 3.22E-02 1.6E+01 0 0 2.7E-01 -4.81E+00 -7.58E-01
GWP-
biogenic kg CO 2 eq -4.75E+00 1.89E-03 2.05E+00 0 9.48E-02 0 1.35E-04 2.42E+00 0 0 5.11E+00 -2.11E-01 -1.93E-01
GWP-luluc kg CO 2 eq 3.36E-02 3.09E-03 5.82E-03 0 1.12E-03 0 2.2E-04 1.25E-03 0 0 2.51E-04 -5.06E-04 -8.02E-05
kg CFC11
ODP 2.48E-09 4.5E-14 3.77E-10 0 5.21E-13 0 3.21E-15 1.57E-11 0 0 4.41E-13 -3.5E-11 -5.55E-12
eq
AP mol H+ eq 1.56E-01 5.12E-04 2.54E-02 0 8.4E-03 0 3.65E-05 5E-03 0 0 1.67E-03 -6.11E-03 -9.66E-04
EP-
kg P eq 1.17E-04 1.64E-06 1.94E-05 0 1.04E-04 0 1.17E-07 4.02E-06 0 0 7.69E-06 -6.98E-06 -1.11E-06
freshwater
EP-marine kg N eq 4.08E-02 1.65E-04 6.72E-03 0 1.77E-03 0 1.18E-05 1.67E-03 0 0 6.01E-04 -1.6E-03 -2.52E-04
EP-terrestrial mol N eq 4.19E-01 1.97E-03 7.02E-02 0 1.53E-02 0 1.41E-04 2.08E-02 0 0 5.78E-03 -1.7E-02 -2.69E-03
kg NMVOC
POCP 1.14E-01 4.41E-04 1.97E-02 2.15E-08 4.98E-03 0 3.15E-05 4.75E-03 0 0 3.04E-03 -4.34E-03 -6.85E-04
eq
ADPE kg Sb eq 2.31E-05 4.62E-08 3.97E-06 0 3.67E-06 0 3.3E-09 3.85E-07 0 0 2.1E-08 -6.52E-07 -1.03E-07
ADPF MJ 6.61E+02 6.01E+00 1.19E+02 0 5.11E+01 0 4.29E-01 2.95E+01 0 0 3.58E+00 -4.34E+01 -6.88E+00
m3 world
WDP eq 6.7E+00 5.13E-03 1.51E+00 0 6.34E-01 0 3.66E-04 1.65E+00 0 0 2.94E-02 -5.45E-01 -8.65E-02
deprived
GWP = Global warming potential; ODP = Depletion potential of the stratospheric ozone layer; AP = Acidification potential of land and water; EP =
Eutrophication potential; POCP = Formation potential of tropospheric ozone photochemical oxidants; ADPE = Abiotic depletion potential for non-fossil
resources; ADPF = Abiotic depletion potential for fossil resources; WDP = Water (user) deprivation potential)
RESULTS OF THE LCA - INDICATORS TO DESCRIBE RESOURCE USE according to EN 15804+A2: 1 m² Wall Panelling System
Parameter Unit A1-A3 A4 A5 B1 B2 C1 C2 C3/1 C3/2 C4/1 C4/2 D/1 D/2
PERE MJ 1.34E+02 4.17E-01 5.3E+01 0 1.85E+00 0 2.98E-02 2.72E+01 0 0 3.76E-01 -2.41E+01 -3.82E+00
PERM MJ 4.35E+01 0 -2.4E+01 0 0 0 0 -1.94E+01 0 0 0 0 0
PERT MJ 1.78E+02 4.17E-01 2.89E+01 0 1.85E+00 0 2.98E-02 7.81E+00 0 0 3.76E-01 -2.41E+01 -3.82E+00
PENRE MJ 5.68E+02 6.04E+00 1.19E+02 0 5.11E+01 0 4.31E-01 1.23E+02 0 0 3.58E+00 -4.34E+01 -6.88E+00
PENRM MJ 9.36E+01 0 0 0 0 0 0 -9.36E+01 0 0 0 0 0
PENRT MJ 6.61E+02 6.04E+00 1.19E+02 0 5.11E+01 0 4.31E-01 2.95E+01 0 0 3.58E+00 -4.34E+01 -6.88E+00
SM kg 1.28E+00 0 1.92E-01 0 0 0 0 0 0 0 0 0 0
RSF MJ 0 0 0 0 0 0 0 0 0 0 0 0 0
NRSF MJ 0 0 0 0 0 0 0 0 0 0 0 0 0
FW m3 1.98E-01 4.82E-04 4.39E-02 0 1.49E-02 0 3.44E-05 4.2E-02 0 0 8.26E-04 -2.3E-02 -3.64E-03
PERE = Use of renewable primary energy excluding renewable primary energy resources used as raw materials; PERM = Use of renewable primary
energy resources used as raw materials; PERT = Total use of renewable primary energy resources; PENRE = Use of non-renewable primary energy
excluding non-renewable primary energy resources used as raw materials; PENRM = Use of non-renewable primary energy resources used as raw
materials; PENRT = Total use of non-renewable primary energy resources; SM = Use of secondary material; RSF = Use of renewable secondary fuels;
NRSF = Use of non-renewable secondary fuels; FW = Use of net fresh water
6 Environmental Product Declaration - Wilsonart - Wall Panelling System
RESULTS OF THE LCA – WASTE CATEGORIES AND OUTPUT FLOWS according to EN 15804+A2:
1 m² Wall Panelling System
Parameter Unit A1-A3 A4 A5 B1 B2 C1 C2 C3/1 C3/2 C4/1 C4/2 D/1 D/2
HWD kg 1.86E-05 3.19E-11 2.79E-06 0 1.7E-04 0 2.28E-12 2.31E-09 0 0 4.28E-10 -3.76E-09 -5.95E-10
NHWD kg 7.77E-01 9.84E-04 1.63E+00 0 1.62E-01 0 7.02E-05 9.9E+00 0 0 8.52E+00 -3.27E-02 -5.18E-03
RWD kg 2.21E-02 1.12E-05 3.67E-03 0 7.93E-04 0 8E-07 9.53E-04 0 0 4.26E-05 -6.94E-03 -1.1E-03
CRU kg 0 0 0 0 0 0 0 0 0 0 0 0 0
MFR kg 1.22E-02 0 1.07E-01 0 0 0 0 0 0 0 0 0 0
MER kg 0 0 0 0 0 0 0 0 0 0 0 0 0
EEE MJ 0 0 5.78E+00 0 0 0 0 1.71E+01 0 0 0 0 0
EET MJ 0 0 1.04E+01 0 0 0 0 3.11E+01 0 0 0 0 0
HWD = Hazardous waste disposed; NHWD = Non-hazardous waste disposed; RWD = Radioactive waste disposed; CRU = Components for re-use;
MFR = Materials for recycling; MER = Materials for energy recovery; EEE = Exported electrical energy; EET = Exported thermal energy
RESULTS OF THE LCA – additional impact categories according to EN 15804+A2-optional:
1 m² Wall Panelling System
Parameter Unit A1-A3 A4 A5 B1 B2 C1 C2 C3/1 C3/2 C4/1 C4/2 D/1 D/2
Disease
PM 2.64E-06 3.52E-09 4.21E-07 0 6.24E-08 0 2.51E-10 1.1E-07 0 0 1.78E-08 -4.96E-08 -7.85E-09
incidence
kBq U235
IR 2.24E+00 1.69E-03 3.8E-01 0 1.3E-01 0 1.21E-04 1.08E-01 0 0 5.8E-03 -1.18E+00 -1.86E-01
eq
ETP-fw CTUe 2.07E+02 4.26E+00 4.33E+01 2.94E-06 7.32E+01 0 3.04E-01 2.44E+01 0 0 1.75E+00 -1.9E+01 -3.01E+00
HTP-c CTUh 7.17E-08 8.78E-11 1.13E-08 2.11E-13 9.85E-10 0 6.27E-12 9.78E-10 0 0 2.07E-10 -7.66E-10 -1.21E-10
HTP-nc CTUh 9.07E-06 4.77E-09 1.41E-06 3.08E-15 7.73E-08 0 3.4E-10 1.03E-07 0 0 2.59E-08 -2.07E-08 -3.28E-09
SQP SQP 8.86E+02 2.55E+00 1.36E+02 0 9.97E-01 0 1.82E-01 6.81E+00 0 0 4.21E-01 -1.56E+01 -2.48E+00
PM = Potential incidence of disease due to PM emissions; IR = Potential Human exposure efficiency relative to U235; ETP-fw = Potential comparative
Toxic Unit for ecosystems; HTP-c = Potential comparative Toxic Unit for humans (cancerogenic); HTP-nc = Potential comparative Toxic Unit for humans
(not cancerogenic); SQP = Potential soil quality index
Disclaimer 1 – for the indicator 'Potential Human exposure efficiency relative to U235'.This impact category deals mainly with the
eventual impact of low-dose ionizing radiation on human health of the nuclear fuel cycle. It does not consider effects due to possible
nuclear accidents, occupational exposure or radioactive waste disposal in underground facilities. Potential ionizing radiation from the
soil, radon and from some construction materials is also not measured by this indicator.
Disclaimer 2 – for the indicators 'abiotic depletion potential for non-fossil resources', 'abiotic depletion potential for fossil resources',
'water (user) deprivation potential, deprivation-weighted water consumption', 'potential comparative toxic unit for ecosystems', 'potential
comparative toxic unit for humans – cancerogenic', 'Potential comparative toxic unit for humans - not cancerogenic', 'potential soil
quality index'. The results of this environmental impact indicator shall be used with care as the uncertainties on these results are high
as there is limited experience with the indicator. This EPD was created using a software tool.
6. LCA: Interpretation
The interpretation is based on the assumptions and limitations individual modules as an example of the global warming
described in the background report, both with regard to the potential.
methods and the data. A dominance analysis is used for
interpretation. The following figure shows the results of the
contributor to the GWP impact, due to combustion emissions.
It is visible that the manufacturing phase dominates the product The GWP impact in the C4/2 module (landfilling scenario) is
system. In addition, the packaging treatment in module A5 has mostly due to the release of the biogenic carbon stored in the
relevant environmental impacts. HPL as both carbon dioxide and methane. Results for module
B2 are declared for the RSL of 20 years.
The C3/1 module (incineration scenario) is the second highest
7 Environmental Product Declaration - Wilsonart - Wall Panelling System
• The GWP-biogenic is shared by the HPL production and
Interpretation of results for the environmental indicators the packaging materials (wood pallets and cardboard)
according to ISO 14044: due to the carbon sequestered in the materials.
• Transportation of raw materials has a relevant influence
• Production of the composite board (a major component
(between 25 % and 50 %) to the AP, EP-marine, EP-
of the wall panel product) has a significant influence
terrestrial and POCP indicators.
(>50 %) on nearly all indicators. It represents more than
• The production process and energy consumption
75 % of the impacts in the GWP-total, ODP, ADPE and
comparatively have minor impacts overall.
water use indicators.
7. Requisite evidence
7.3. Non-wood based substrate covered with a decorative layer
VOC and formaldehyde emissions 7.3.1 Formaldehyde
Determination of the VOC and formaldehyde emission Measurement of the specific migration according to DIN
according to/compliance with AgBB-Scheme / ISO 16000 part CEN/TS 13130-23:2005 Materials and items with contact to
3, 6 and 9 food –
Substances in plastics which are subject to restrictions. Limit
Measurement centre: Eurofins Product Testing A/S- values
Smedeskovvej 38 -8464 Galten - Denmark as per the German Consumer Goods Ordinance (2005) and
EU Directive
Test report: 392-2019-00131801-A-EN-03 of 02.04.2019 10/2011/EC
Result: 7.3.2 Total migration
A rating according to the regulation of March and May 2011 - Measurement to
tested according to a wall scenario with a loading factor of 1.0 the standard series EN 1186, Limit values as per the German
m2/m3 Consumer Goods
Formaldehyde E1 class - formaldehyde result based on Ordinance (2005) and EU Directive 10/2011/EC.
chamber testing and DNPH sampling according to ISO 16000.
The result is therefore not directly according to EN 717-1, and 7.3.3 For products used in indoor applications.
there are a few small deviations. The testing is in accordance Test method in accordance with the AgBB schema
with the conclusions presented in CEN TC351 WG2 N174 indicating the measuring agency, date and results as a
where the difference and compatibility between EN 717-1 and range of values. Evidence of VOC is optional when the
ISO 16000 are empirically and theoretically analysed. EPD is valid for a shorter period of time (1 year). At
least the following must be declared:
AgBB overview of results (28 days [µg/m³])
AgBB overview of results (3 days [µg/m³])
Name Value Unit
TVOC (C6 - C16) 10 μg/m3 Name Value Unit
Sum SVOC (C16 - C22) < 5 μg/m3
TVOC (C6 - C16) 20 μg/m3
Sum SVOC (C16 - C22) < 5 μg/m3
R (dimensionless) 170 -
VOC without NIK < 5 μg/m3 R (dimensionless) 250 -
Carcinogenic Substances < 1 μg/m3
VOC without NIK < 5 μg/m3
Carcinogenic Substances < 1 μg/m3
Formaldehyde 16 µg/m3
8. References
Standards
EN 15804
EN 438 : High-pressure decorative laminates (HPL) - EN15804:2012+A2:2019+AC:2021, Sustainability of
Sheets based on thermosetting resins (usually called construction works —Environmental Product Declarations —
laminates) Core rules for the product category of construction products.
EN438-2:2016 : Part 2: Determination of properties
EN438-3:2016: Part 3 : classification and specifications for ISO 9001
laminates less than 2 mm thick intended for bonding to ISO 9001: 2015: Quality Management System
supporting substrates
EN438-7 : 2005 :Part 7: Compact laminate and HPL composite ISO 13894
panels for internal and external wall and ceiling finishes ISO 13894 : High-pressure decorative laminate - Composite
elements - Part 1 : test methods - part 2 : specifications
EN 717-1
EN 717-1: 2004:Wood-based panels. Determination of ISO 14001
formaldehyde release Formaldehyde emission by the chamber ISO 14001: 2015: Environmental Management System
method
ISO 14025
EN ISO 14025:2011, Environmental labels and declarations —
EN 13501-1 Type III environmental
EN13501-1: Fire classification of construction products and declarations — Principles and procedures.
building elements -
Part 1 : classification using data from reaction to fire tests ISO 16000
8 Environmental Product Declaration - Wilsonart - Wall Panelling System
ISO 16000: Indoor air - Part 3 : determination of formaldehyde - databases, LBP, University of
Part 6 : Stuttgart and Sphera Solutions GmbH, Leinfelden-
determination of organic compounds - Part 9 : determination of Echterdingen, 2021.
the (http://www.gabi-software.com/support/gabi/gabi[1]database-
emission of volatile organic compounds from building products 2021-lci-documentation/)
and
furnishing - Emission test chamber method IBU 2021
Institut Bauen und Umwelt e.V.: General Instructions for the
NFP 92-501 EPD programme of Institut
NFP 92-501 : Safety against fire - Building materials - Reaction Bauen und Umwelt e.V., Version 2.0, Berlin: Institut Bauen und
to fire tests Umwelt e.V., 2021 www.ibu-epd.com
Further References PCR Part A
PCR - Part A: Calculation rules for the Life Cycle Assessment
BBSR and Requirements on the
BBSR table (german): 'Nutzungsdauern von Bauteilen zur Background Report, version 1.6, Institut Bauen und Umwelt
Lebenszyklusanalyse nach e.V.,
BNB', Bundesinstitut für Bau-, Stadt- und Raumforschung, www.bau-umwelt.com, 2017
Referat II Nachhaltiges Bauen; online available under
https://www.nachhaltigesbauen.de/austausch/nutzungsdauernvon- PCR Part B
auteilen/ Part B: Requirements on the EPD for Decorative board for
interior use , 09/2022
REACH
BPR Regulation (EC) No 1907/2006 concerning the Registration,
BPR : Biocidal Products Evaluation, Authorisation and
Regulation (BPR) refers to Regulation (EU) 528/2012 Restriction of Chemicals (REACH)
concerning the
placing on the market and use of biocidal products. Regulation (EU) No 305/2011
Regulation (EU) No 305/2011 of the European Parliament and
GaBi of the Council of 9 March 2011 laying down harmonised
GaBi Software System and Database for Life Cycle conditions for the marketing of construction products and
Engineering, 1992-2021, Sphera repealing Council Directive 89/106/EEC
Solutions GmbH, Leinfelden-Echterdingen, with
acknowledgement of LBP University European Waste Catalogue
of Stuttgart, program version GaBi 10; database version 2022.1 Guidance on Classification of Waste according to EWC-stat
categories version 2, December 2010
GaBi documentation
GaBi dataset documentation for the software system and
9 Environmental Product Declaration - Wilsonart - Wall Panelling System
Publisher
Institut Bauen und Umwelt e.V. +49 (0)30 3087748- 0
Hegelplatz 1 info@ibu-epd.com
10117 Berlin www.ibu-epd.com
Germany
Programme holder
Institut Bauen und Umwelt e.V. +49 (0)30 3087748- 0
Hegelplatz 1 info@ibu-epd.com
10117 Berlin www.ibu-epd.com
Germany
Author of the Life Cycle Assessment
Sphera Solutions GmbH +49 711 341817-0
Hauptstraße 111- 113 info@sphera.com
70771 Leinfelden-Echterdingen www.sphera.com
Germany
Owner of the Declaration
WILSONART +44 1933 232200
Rixon Road 9-29 businesssupport@bushboard.co.uk
NN8 4B Wellingborough, Northamptonshire www.bushboard.co.uk
United Kingdom
POLYREY +33 (0)5 53 63 80 80
Route de Bergerac 700 support.technique@polyrey.com
24150 Baneuil www.polyrey.com
France
10 Environmental Product Declaration - Wilsonart - Wall Panelling System
