ENVIRONMENTAL PRODUCT DECLARATION
as per ISO 14025 and EN 15804+A1
Owner of the Declaration Interface Europe Manufacturing BV
Programme holder Institut Bauen und Umwelt e.V. (IBU)
Publisher Institut Bauen und Umwelt e.V. (IBU)
Declaration number EPD-INT-20200181-CCC1-EN
Issue date 05.11.2020
Valid to 04.11.2025
Modular carpet tiles with CQuest Bio backing
pile material solution-dyed polyamide 6 with 100% recycled
content and a maximum total pile weight of 1500 g/m2
Interface®
www.ibu-epd.com | https://epd-online.com
Umwelt Produktdeklaration Name des Herstellers – Name des Produkts
General Information
Interface® Modular carpet tiles with CQuest
Bio backing
pile material solution-dyed PA 6 with
100% recycled content and a max.
total pile weight of 1500 g/m2
Programme holder Owner of the declaration
IBU – Institut Bauen und Umwelt e.V. Interface Europe Manufacturing BV
Panoramastr. 1 Industrielaan 15
10178 Berlin 3925 ZG Scherpenzeel
Germany The Netherlands
Declaration number Declared product / declared unit
EPD-INT-20200181-CCC1-EN 1 m² tufted modular carpet tiles with CQuest Bio
backing (CQB) and a pile material of PA 6 with 100%
recycled content
This declaration is based on the product Scope:
category rules: The manufacturer declaration applies to modular
Floor coverings, 02/2018 carpet tiles with CQuest Bio backing, a pile material of
(PCR checked and approved by the SVR) PA 6 with 100% recycled content and a maximum total
pile weight of 1500 g/m2. The products are tufted in
Scherpenzeel, The Netherlands, or in Craigavon,
Issue date
Ireland. They are back coated in Scherpenzeel.
05.11.2020
LCA results for products with a maximum total pile
weight of 600 g/m2 can be taken from the
Valid to
corresponding tables of the annexe. Specific data for
04.11.2025 every product within the declared group of products in
relation to its total pile weight can be calculated by
using equation 1 given in the annexe (see annexe
chapter: 'General Information on the annexe').
The declaration is only valid in conjunction with a valid
GUT-PRODIS license of the product.
The owner of the declaration shall be liable for the
underlying information and evidence; the IBU shall not
be liable with respect to manufacturer information, life
cycle assessment data and evidences.
The EPD was created according to the specifications
of EN 15804+A1. In the following, the standard will be
simplified as EN 15804.
Verification
The standard EN 15804 serves as the core PCR
Independent verification of the declaration and data
according to ISO 14025:2010
Dipl. Ing. Hans Peters internally x externally
(chairman of Institut Bauen und Umwelt e.V.)
Dr. Alexander Röder Dr. Frank Werner
(Managing Director Institut Bauen und Umwelt e.V.)) (Independent verifier)
Product
Information about the enterprise way that is restorative to the planet and creates a
Interface, Inc. is a global flooring company specializing climate fit for life.
in carbon neutral carpet tile and resilient flooring,
including luxury vinyl tile (LVT) and nora® rubber Product description/Product definition
flooring. We help our customers create high- Tufted modular carpet tiles having a surface pile of
performance interior spaces that support well-being, solution-dyed polyamide 6 with 100% recycled content
productivity, and creativity, as well as the sustainability and a CQuest Bio backing system.
of the planet. Our mission, Climate Take Back™,
invites you to join us as we commit to operating in a
2 Environmental Product Declaration Interface – Tufted modular carpet tiles with CQuest Bio backing and a pile material of
PA 6 with 100% recycled content
CQuest Bio backing system: Backing compound based
on wood resin, containing a recycled filler, glass-fleece
reinforcement and polypropylene covering fleece. Performance data of the product in accordance with
The minimum recycled content out of total weight is the declaration of performance with respect to its
81% with a total pile weight of 1500 g/m2. essential characteristics according to EN 14041.
The declaration applies to a group of products with a Additional product properties in accordance with EN
maximum total pile weight of 1500 g/m2. 1307 can be found on the Product Information System
LCA results for products with a maximum total pile PRODIS using the PRODIS registration number of the
weight of 600 g/m2 can be taken from the product (www.pro-dis.info) or on the manufacturer's
corresponding tables of the annexe. technical information section (www.interface.com).
Results for specific products with any other total pile
weight can be calculated by using equation 1 given in Base materials/Ancillary materials
the annexe (see annexe chapter: 'General Information
on the annexe'). Name Value Unit
For the placing on the market of the product in the Polyamide 6 27.9 %
European Union/European Free Trade Association Polyester 2.2 %
(EU/EFTA) (with the exception of Switzerland) Polypropylene 0.9 %
Regulation (EU) No. 305/2011 Construction Product Limestone 47.8 %
Regulation (CPR) applies. The product needs a Aluminum hydroxide 6.3 %
Declaration of Performance (DoP) taking into Ethylene vinyl acetate (EVA) 7.0 %
consideration EN 14041 and the CE-marking. The DoP Wood resin 5.4 %
of the product can be found on the manufacturer's
Glass fibre 0.6 %
technical information section. For the application and
Additives 1.9 %
use of the product the respective national provisions
apply.
The products are registered in the GUT-PRODIS
Information System. The PRODIS system ensures the
Application
compliance with limitations of various chemicals and
According to the use class as defined in EN 1307 the
Volatile Organic Compound (VOC)-emissions and a
products can be used in all professional areas which
ban on the use of all substances that are listed as
require class 33 or less.
'Substances of Very High Concern' (SVHC) under
REACH.
This product contains substances listed in the ECHA
candidate list (27.06.2018) exceeding 0.1 percentage
by mass: no
Technical Data
The performance data listed in the DoP apply.
Reference service life
Name Value Unit A calculation of the reference service life according to
Modular carpet tiles, ISO 15686 is not possible.
Product Form -
50 cm x 50 cm The service life of textile floor coverings strongly
Type of manufacture tufted carpet - depends on the correct installation taking into account
PA6 with 100% recycled the declared use classification and the adherence to
Yarn type -
content cleaning and maintenance instructions.
Colouration solution-dyed yarn A minimum service life of 10 years can be assumed,
PET with 88 % recycled technical service life can be considerably longer.
Primary
content
CQuest Bio backing, heavy
Secondary backing -
backing with textile bottom
Total pile weight 1500 g/m²
Total carpet weight 5380 g/m2
LCA: Calculation rules
Declared Unit
System boundaries of modules A, B, C, D:
Modules C3, C4 and D are indicated separately for
Name Value Unit three end-of-life scenarios:
Declared unit 1 m2 - 1 landfill disposal
Conversion factor to 1 kg 5.38 - - 2 municipal waste incineration
Mass reference 5.38 kg/m² - 3 recovery in a cement plant
The declared unit refers to 1 m2 produced textile floor
covering. The output of module A5 'Assembly' is 1 m2 A1-A3 Production:
installed textile floor covering. Energy supply and production of the basic material,
processing of secondary material, auxiliary material,
transport of the material to the manufacturing site,
System boundary emissions, waste water treatment, packaging material
and waste processing up to the landfill disposal of
Type of EPD: Cradle-to-grave residual waste (except radioactive waste). Benefits for
3 Environmental Product Declaration Interface – Tufted modular carpet tiles with CQuest Bio backing and a pile material of
PA 6 with 100% recycled content
generated electricity and steam due to the incineration C2 Transport:
of production waste are aggregated. Transport of the carpet waste to a landfill, to the
Biogenic carbon that is stored in renewable material municipal waste incineration plant (MWI) or to the
(wood resin, renewable additives, packaging paper) is waste collection facility for recycling.
taken into account as well as the associated carbon
dioxide uptake from the air from which this biogenic C3 Waste processing:
carbon comes. C3-1: Landfill disposal needs no waste processing.
C3-2: The impact from waste incineration (plant with
A4 Transport: R1>0.6), generated electricity and steam are listed in
Transport of the packed textile floor covering the result table as exported energy. The biogenic
from factory gate to the place of installation. carbon that is stored in the renewable materials of the
floor covering is released into the air as carbon dioxide
A5 Installation: emissions.
Installation of the textile floor covering, processing of C3-3: Collection of the carpet waste for recovery in the
installation waste and packaging waste up to the cement industry, waste processing (granulating),
landfill disposal of residual waste (except radioactive transport to the cement plant, emissions from the
waste), the production of the amount of carpet that incineration. The biogenic carbon that is stored in the
occurs as installation waste including its transport to renewable materials of the floor covering is released
the place of installation. Generated electricity and into the air as carbon dioxide emissions.
steam due to the incineration of waste are listed in the
result table as exported energy. C4 Disposal
Biogenic carbon that is stored in renewable materials C4-1: Impact from landfill disposal. The biogenic
in installation waste and packaging paper is released carbon that is stored in the renewable materials of the
as carbon dioxide emissions into the air at the end of floor covering is released into the air as carbon dioxide
life in module A5. emissions.
Preparation of the floor and auxiliary materials C4-2: The carpet waste leaves the system in
(adhesives, fixing agents, PET connectors) are beyond module C3-2.
the system boundaries and not taken into account. C4-3: The pre-processed carpet waste leaves the
system in module C3-3.
B1 Use:
Indoor emissions during the use stage. After the first D Recycling potential:
year, no product- related Volatile Organic Compound Calculated benefits result from materials exclusive
(VOC) emissions are relevant due to known VOC secondary materials (net materials).
decay curves of the product.
D-A5: Benefits for generated energy due
B2 Maintenance: to incineration of packaging and installation waste
Cleaning of the textile floor covering for a period of 1 (incineration plant with R1 > 0.6),
year: D-1: Benefits for generated energy due to landfill
Vacuum cleaning – electricity supply. disposal of carpet waste at the end-of-life,
Wet cleaning – electricity, water consumption, D-2: Benefits for generated energy due to incineration
production of the cleaning agent, waste water of carpet waste at the end-of-life (incineration plant
treatment. with R1 > 0.6),
The declared values in this module have to be D-3: Benefits for saved fossil energy and saved
multiplied by the assumed service life of the floor inorganic material due to recovery of the carpet in a
covering in the building in question. cement plant.
B3 - B7: Comparability
The modules are not relevant and therefore not Basically, a comparison or an evaluation of EPD data
declared. is only possible if all the data sets to be compared
were created according to EN 15804 and the building
C1 De-construction: context, respectively the product-specific
The floor covering is de-constructed manually and no characteristics of performance, are taken into account.
additional environmental impact is caused.
Background data are taken from the GaBi database
2020, service pack 40. Remaining data gaps are
covered by the ecoinvent 3.6 database 2019.
LCA: Scenarios and additional technical information
The following information refer to the declared modules
and are the basis for calculations or can be used for Installation in the building (A5)
further calculations. The indicated values refer to the Name Value Unit
declared functional unit of all products with a total pile Material loss 0.16 kg
weight up to 1500 g/m2. Polyethene packaging waste and installation waste are
considered to be incinerated in a municipal waste
Transport to the construction site (A4) incineration plant. Cardboard packaging waste is going
Name Value Unit to be recycled.
Litres of fuel (truck, EURO 0-6 mix) 0.0126 l/100km Preparation of the floor and auxiliaries (adhesives,
Transport distance 700 km fixing agents, PET connectors, etc.) are not taken into
Capacity utilisation (incl. empty runs) 55 % account.
4 Environmental Product Declaration Interface – Tufted modular carpet tiles with CQuest Bio backing and a pile material of
PA 6 with 100% recycled content
Maintenance (B2)
The values for cleaning refer to 1 m2 floor covering
used in commercial areas per year. Depending on the
application based on ISO 10874, the technical service
life recommended by the manufacturer and the
anticipated strain on the floor by customers, the case-
specific useful life can be established. Based on this
useful life the effects of Module B2 need to be
calculated in order to obtain the overall environmental
impacts.
Name Value Unit
Maintenance cycle (wet cleaning) 1.5 1/year
Maintenance cycle (vacuum
208 1/year
cleaning)
Water consumption (wet cleaning) 0.004 m3
Cleaning agent (wet cleaning) 0.09 kg
Electricity consumption 0.314 kWh
Further information on cleaning and maintenance see
www.interface.com
End of Life (C1-C4)
Three different end-of-life scenarios are declared and
the results are indicated separately in module C.
Each scenario is calculated as a 100% scenario.
Scenario 1: 100% landfill disposal
Scenario 2: 100% municipal waste incineration (MWI)
with R1>0.6
Scenario 3: 100% recycling in the cement industry
If combinations of these scenarios have to be
calculated this should be done according to the
following scheme:
EOL-impact = x% impact (Scenario 1)
+ y% impact (Scenario 2)
+ z% impact (Scenario 3)
with x% + y% + z% = 100%
Name Value Unit
Collected as mixed construction waste
5.38 kg
(scenario 1 and 2)
Collected separately (scenario 3) 5.38 kg
Landfilling (scenario 1) 5.38 kg
Energy recovery (scenario 2) 5.38 kg
Energy recovery (scenario 3) 2.434 kg
Recycling (scenario 3) 2.946 kg
Reuse, recovery and/or recycling potentials (D),
relevant scenario information
Recovery or recycling potentials due to the three end-
of-life scenarios (module C) are indicated separately.
Recycling in the cement industry (scenario 3)
VDZ e.V.
The organic material of the carpet is used as
alternative fuel in a cement kiln. It mainly substitutes
for lignite (64.5%), hard coal (26.5%) and petrol coke
(9.0%).
The inorganic material is substantially integrated into
the cement clinker and substitutes for original material
input.
5 Environmental Product Declaration Interface – Tufted modular carpet tiles with CQuest Bio backing and a pile material of
PA 6 with 100% recycled content
LCA: Results
The LCA results refer to all declared products with a maximum total pile weight of 1500 g/m2.
LCA results for products with a maximum total pile weight of 600 g/m2 can be taken from the corresponding tables
of the annexe. Results for specific products with any other total pile weight can be calculated by using equation 1
given in the annexe (see annexe chapter: 'General Information on the annexe'). The declared result figures in
module B2 have to be multiplied by the assumed service life (in years) of the floor covering in the building under
consideration.
Information on un-declared modules: Modules B6, B7, C1, C3/1, C4/2 and C4/3 cause no additional impact (see
chapter "LCA: Calculation rules" in this document) and are not relevant. They are marked as 'modules not
declared' (MND). Module C2 represents the transport for scenarios 1, 2 and 3. Column D represents module
D/A5. The calculations are based on the CML characterization factors (version January 2016).
DESCRIPTION OF THE SYSTEM BOUNDARY (X = INCLUDED IN LCA; MND = MODULE NOT DECLARED;
MNR = MODULE NOT RELEVANT)
BENEFITS AND
CONSTRUCTI LOADS
PRODUCT STAGE ON PROCESS USE STAGE END OF LIFE STAGE BEYOND THE
STAGE SYSTEM
BOUNDARIES
6 Environmental Product Declaration Interface – Tufted modular carpet tiles with CQuest Bio backing and a pile material of
PA 6 with 100% recycled content
lairetam
waR
ylppus tropsnarT
gnirutcafunaM
eht
morf
tropsnarT
etis
eht
ot
etag
ylbmessA esU
ecnanetniaM
riapeR
tnemecalpeR tnemhsibrufeR
ygrene
lanoitarepO esu
retaw
lanoitarepO esu
noitcurtsnoc-eD
noitilomed tropsnarT
gnissecorp
etsaW
lasopsiD -esueR -yrevoceR -gnilcyceR laitnetop
A1 A2 A3 A4 A5 B1 B2 B3 B4 B5 B6 B7 C1 C2 C3 C4 D
X X X X X X X MNR MNR MNR MND MND MND X X X X
RESULTS OF THE LCA - ENVIRONMENTAL IMPACT according to EN 15804+A1: 1 m² floorcovering
Parameter Unit A1-A3 A4 A5 B1 B2 C2 C3/2 C3/3 C4/1 D D/1 D/2 D/3
GWP [kg CO2-Eq.] 5.46E+0 3.19E-1 6.00E-1 0.00E+0 2.92E-1 1.78E-2 7.08E+0 7.16E+0 1.26E+0 -1.74E-2 0.00E+0 -2.52E-1 -2.51E-1
-2.44E- -3.46E- -1.47E-
ODP [kg CFC11-Eq.] 4.45E-8 5.24E-17 1.34E-9 0.00E+0 1.21E-8 2.93E-182.47E-153.36E-151.18E-15 0.00E+0
16 15 15
AP [kg SO2-Eq.] 2.02E-2 1.35E-3 8.00E-4 0.00E+0 1.16E-3 7.51E-5 4.95E-3 5.20E-3 9.84E-4 -2.19E-5 0.00E+0 -3.12E-4 -9.80E-4
EP [kg (PO4)3--Eq.] 1.22E-2 3.38E-4 4.13E-4 0.00E+0 3.17E-4 1.89E-5 1.24E-3 1.29E-3 1.03E-3 -2.73E-6 0.00E+0 -3.91E-5 -1.20E-4
POCP [kg ethene-Eq.] 1.25E-3 -5.66E-4 2.83E-5 6.29E-5 1.48E-4 -3.16E-5 3.00E-4 2.25E-4 1.11E-4 -2.00E-6 0.00E+0 -2.88E-5 -8.71E-5
ADPE [kg Sb-Eq.] 1.26E-5 2.69E-8 3.87E-7 0.00E+0 4.43E-6 1.50E-9 2.30E-7 2.43E-7 7.02E-8 -3.24E-9 0.00E+0 -4.61E-8 -1.90E-7
ADPF [MJ] 9.79E+1 4.35E+0 3.19E+0 0.00E+0 6.76E+0 2.43E-1 3.73E+0 4.66E+0 5.41E+0 -2.45E-1 0.00E+0-3.56E+0-2.31E+1
GWP = Global warming potential; ODP = Depletion potential of the stratospheric ozone layer; AP = Acidification potential of land and water; EP =
Caption Eutrophication potential; POCP = Formation potential of tropospheric ozone photochemical oxidants; ADPE = Abiotic depletion potential for non-
fossil resources; ADPF = Abiotic depletion potential for fossil resources
RESULTS OF THE LCA - INDICATORS TO DESCRIBE RESOURCE USE according to EN 15804+A1: 1 m²
floorcovering
Parameter Unit A1-A3 A4 A5 B1 B2 C2 C3/2 C3/3 C4/1 D D/1 D/2 D/3
PERE [MJ] 7.10E+1 2.45E-1 2.90E+0 0.00E+0 1.20E+0 1.37E-2 1.39E+1 1.41E+1 3.92E-1 -6.51E-2 0.00E+0 -9.21E-1 -3.45E-1
PERM [MJ] 1.36E+1 0.00E+0 -3.39E-1 0.00E+0 0.00E+0 0.00E+0 -1.33E+1 -1.33E+1 0.00E+0 0.00E+0 0.00E+0 0.00E+0 0.00E+0
PERT [MJ] 8.47E+1 2.45E-1 2.57E+0 0.00E+0 1.20E+0 1.37E-2 5.83E-1 8.52E-1 3.92E-1 -6.51E-2 0.00E+0 -9.21E-1 -3.45E-1
PENRE [MJ] 9.27E+1 4.36E+0 3.66E+0 0.00E+0 7.86E+0 2.43E-1 1.53E+1 1.64E+1 5.58E+0 -3.01E-1 0.00E+0 -4.35E+0 -2.34E+1
PENRM [MJ] 1.15E+1 0.00E+0 -2.69E-1 0.00E+0 0.00E+0 0.00E+0 -1.12E+1 -1.12E+1 0.00E+0 0.00E+0 0.00E+0 0.00E+0 0.00E+0
PENRT [MJ] 1.04E+2 4.36E+0 3.39E+0 0.00E+0 7.86E+0 2.43E-1 4.09E+0 5.23E+0 5.58E+0 -3.01E-1 0.00E+0 -4.35E+0 -2.34E+1
SM [kg] 4.40E+0 0.00E+0 1.32E-1 0.00E+0 0.00E+0 0.00E+0 0.00E+0 0.00E+0 0.00E+0 0.00E+0 0.00E+0 0.00E+0 2.60E-1
RSF [MJ] 0.00E+0 0.00E+0 0.00E+0 0.00E+0 0.00E+0 0.00E+0 0.00E+0 0.00E+0 0.00E+0 0.00E+0 0.00E+0 0.00E+0 0.00E+0
NRSF [MJ] 0.00E+0 0.00E+0 0.00E+0 0.00E+0 0.00E+0 0.00E+0 0.00E+0 0.00E+0 0.00E+0 0.00E+0 0.00E+0 0.00E+0 0.00E+0
FW [m³] 4.93E-1 2.83E-4 1.54E-2 0.00E+0 4.27E-3 1.58E-5 2.04E-2 2.08E-2 6.85E-5 -7.54E-5 0.00E+0 -1.07E-3 -2.19E-3
PERE = Use of renewable primary energy excluding renewable primary energy resources used as raw materials; PERM = Use of
renewable primary energy resources used as raw materials; PERT = Total use of renewable primary energy resources; PENRE = Use of
non-renewable primary energy excluding non-renewable primary energy resources used as raw materials; PENRM = Use of non-
Caption
renewable primary energy resources used as raw materials; PENRT = Total use of non-renewable primary energy resources; SM = Use
of secondary material; RSF = Use of renewable secondary fuels; NRSF = Use of non-renewable secondary fuels; FW = Use of net fresh
water
RESULTS OF THE LCA – WASTE CATEGORIES AND OUTPUT FLOWS according to EN 15804+A1:
1 m² floorcovering
Parameter Unit A1-A3 A4 A5 B1 B2 C2 C3/2 C3/3 C4/1 D D/1 D/2 D/3
HWD [kg] 6.81E-3 2.03E-7 2.04E-4 0.00E+0 9.63E-10 1.13E-8 1.90E-8 4.75E-8 2.04E-8 -1.20E-10 0.00E+0 -1.73E-9 -5.89E-9
NHWD [kg] 1.72E+0 6.67E-4 9.61E-2 0.00E+0 5.63E-3 3.72E-5 1.48E+0 1.48E+0 5.36E+0 -1.38E-4 0.00E+0 -1.98E-3 -1.62E-1
RWD [kg] 2.11E-3 5.40E-6 6.79E-5 0.00E+0 3.38E-4 3.01E-7 1.44E-4 2.25E-4 6.74E-5 -2.22E-5 0.00E+0 -3.15E-4 -8.94E-5
CRU [kg] 0.00E+0 0.00E+0 0.00E+0 0.00E+0 0.00E+0 0.00E+0 0.00E+0 0.00E+0 0.00E+0 0.00E+0 0.00E+0 0.00E+0 0.00E+0
MFR [kg] 0.00E+0 0.00E+0 1.21E-1 0.00E+0 0.00E+0 0.00E+0 0.00E+0 1.70E+0 0.00E+0 0.00E+0 0.00E+0 0.00E+0 0.00E+0
MER [kg] 0.00E+0 0.00E+0 0.00E+0 0.00E+0 0.00E+0 0.00E+0 0.00E+0 0.00E+0 0.00E+0 0.00E+0 0.00E+0 0.00E+0 0.00E+0
EEE [MJ] 0.00E+0 0.00E+0 2.79E-1 0.00E+0 0.00E+0 0.00E+0 7.88E+0 0.00E+0 0.00E+0 0.00E+0 0.00E+0 0.00E+0 0.00E+0
EET [MJ] 0.00E+0 0.00E+0 5.18E-1 0.00E+0 0.00E+0 0.00E+0 1.47E+1 8.41E+1 0.00E+0 0.00E+0 0.00E+0 0.00E+0 0.00E+0
HWD = Hazardous waste disposed; NHWD = Non-hazardous waste disposed; RWD = Radioactive waste disposed; CRU = Components
Caption for re-use; MFR = Materials for recycling; MER = Materials for energy recovery; EEE = Exported electrical energy; EEE = Exported
thermal energy
Information on the biogenic carbon content: The textile floor covering contains renewable materials with stored
biogenic carbon. During the growth phase of plants carbon dioxide (CO ) is absorbed and transformed into stored
2
biogenic carbon. This amount of CO uptake is taken into account in module A1-A3 as a negative value that
2
reduces the total amount of the GWP. At the end of life the same amount of CO is released into the air as
2
emissions. These CO emissions increase the amount of the GWP in the three scenarios landfill disposal,
2
municipal incineration and recovery in the cement industry.
Biogenic carbon content per m2 textile floor covering: 0.27 kg C
Corresponding carbon dioxide uptake/emissions: 0.99 kg CO
2
Not all of the life cycle inventories applied in this study support the methodological approach for the waste and
water indicators. The data are based on publications of industry. The indicators for waste and water of the system
are evaluated but contain a higher degree of uncertainty.
References
EN 1307 ECHA candidate list
DIN EN 1307: 2014+A1:2016: Textile floor coverings - Candidate List of substances of very high concern
Classification (SVHCs) for authorisation, 16.01.2020, European
EN 13501-1 Chemicals Agency (ECHA), Helsinki, Finland
DIN EN 13501-1:2010-01: Fire classification of ecoinvent 3.6
construction products and building elements - Part 1: ecoinvent, Zurich, Switzerland, database version 3.6,
Classification using data from reaction to fire tests published September 2019
EN 14041 GaBi database 2020
DIN EN 14041: 2018-05: Resilient, textile and laminate GaBi Software-System and Database for Life Cycle
floor coverings - Essential characteristics Engineering, thinkstep AG, Leinfelden-Echterdingen,
EN 15804 service pack 40, 2020
EN 15804:2012-04+A1 2013/, Sustainability of IBU 2016
construction works — Environmental Product IBU (2016): General Programme Instructions for the
Declarations — Core rules for the product category of Preparation of EPDs at the Institut Bauen und Umwelt
construction products e.V., Version 1.1 Institut Bauen und Umwelt e.V.,
EN 16810 Berlin, www.ibu-epd.de
DIN EN 16810: 2017-08: Resilient, textile and laminate PCR Part A
floor coverings – Environmental product declarations – Product Category Rules for Construction Products
Product category rules from the range of Environmental Product Declarations.
ISO 10874 Part A: Calculation Rules for the Life Cycle
DIN EN ISO 10874: 2012-04: Resilient, textile and Assessment and Requirements on the Background
laminate floor coverings - Classification Report, V1.8, Berlin: Institut Bauen und Umwelt e.V.
ISO 14025 (IBU), July 2019
DIN EN /ISO 14025:2011-10: Environmental labels PCR Part B
and declarations — Type III environmental Product Category Rules for Construction Products
declarations — Principles and procedures from the range of Environmental Product Declarations
ISO 15686 of Institut Bauen und Umwelt (IBU), Part B: Require-
ISO 15686: Buildings and constructed assets - ments on the EPD for floor coverings, V1.2, Berlin:
Service life planning Institut Bauen und Umwelt e.V. (IBU), February 2018
ISO 15686-1: 2011-05: Part 1: General principles and PRODIS
framework Product Information System (PRODIS) of the
ISO 15686-2: 2012-05: Part 2: Service life prediction European Carpet Industry, Gemeinschaft
procedures umweltfreundlicher Teppichboden e.V (GUT) and
ISO 15686-7: 2006-03: Part 7: Performance European Carpet and Rug Association
evaluation for feedback of service life data (ECRA), http://www.pro-dis.info
from practice REACH
ISO 15686-8: 2008-06: Part 8: Reference service life Regulation (EC) No 1907/2006 of the European
and service-life estimation Parliament and of the Council of 18 December 2006
Regulation (EU) No. 305/2011 concerning the Registration, Evaluation, Authorisation
Regulation No. 305/2011 Construction Products and Restriction of Chemicals (REACH). Last update:
Regulation (CPR) of the European Council and of the 25.03.2014 (Status: 27.06.2018)
European Parliament, April 2011 VDZ e.V.
CML characterization factors Association of German Cement Works, Ed. Environ-
Impact assessment characterization factors, Institute of mental Data of the German Cement Industry 2018
Environmental Sciences - in Dutch 'Centrum voor
Milieuwetenschappen in Leiden' (CML), Leiden, The
Netherlands
7 Environmental Product Declaration Interface – Tufted modular carpet tiles with CQuest Bio backing and a pile material of
PA 6 with 100% recycled content
Publisher
Institut Bauen und Umwelt e.V. Tel +49 (0)30 3087748- 0
Panoramastr. 1 Fax +49 (0)30 3087748- 29
10178 Berlin Mail info@ibu-epd.com
Germany Web www.ibu-epd.com
Programme holder
Institut Bauen und Umwelt e.V. Tel +49 (0)30 - 3087748- 0
Panoramastr 1 Fax +49 (0)30 – 3087748 - 29
10178 Berlin Mail info@ibu-epd.com
Germany Web www.ibu-epd.com
Author of the Life Cycle
Assessment Tel +49 (0)241 96843 410
Gemeinschaft umweltfreundlicher Fax +49 (0)241 96843 400
Teppichboden (GUT) e.V. Mail mail@gut-ev.de
Schönebergstraße 2 Web www.gut-ev.org
52068 Aachen
Germany
Owner of the Declaration
Interface Europe Manufacturing Tel +31 33 277 55 55
BV Fax +31 33 277 55 54
Industrielaan 15 Mail receptie@interface.com
3925ZG Scherpenzeel Web www.interface.com
Netherlands
