ENVIRONMENTAL PRODUCT DECLARATION
as per ISO 14025 and EN 15804+A2
Owner of the Declaration Knauf Gips KG
Publisher Institut Bauen und Umwelt e.V. (IBU)
Programme holder Institut Bauen und Umwelt e.V. (IBU)
Declaration number EPD-KNA-20230213-IBB1-EN
Issue date 10/04/2024
Valid to 09/04/2029
Knauf Silentboard GKF
Knauf Gips KG
www.ibu-epd.com | https://epd-online.com
1. General Information
Knauf Gips KG Knauf Silentboard GKF
Programme holder Owner of the declaration
IBU – Institut Bauen und Umwelt e.V. Knauf Gips KG
Hegelplatz 1 Am Bahnhof 7
10117 Berlin 97346 Iphofen
Germany Germany
Declaration number Declared product / declared unit
EPD-KNA-20230213-IBB1-EN Plasterboard Knauf Silentboard Type GKF according to DIN 18180
respectively DF according to EN 520, 1 m², board thickness 12.5 mm,
weight of board 17.5 kg/m²
This declaration is based on the product category rules: Scope:
Plasterboard, 01/08/2021 This EPD covers 100 % of manufacture of the plasterboard Knauf
(PCR checked and approved by the SVR) Silentboard GKF. This plasterboard is manufactured in plant Iphofen
(Germany). The life cycle assessment is based on production data for year
2022.
Issue date The owner of the declaration shall be liable for the underlying information
and evidence; the IBU shall not be liable with respect to manufacturer
10/04/2024
information, life cycle assessment data and evidences.
The EPD was created according to the specifications of EN 15804+A2. In
Valid to
the following, the standard will be simplified as EN 15804.
09/04/2029
Verification
The standard EN 15804 serves as the core PCR
Independent verification of the declaration and data according to ISO
14025:2011
internally X externally
Dipl.-Ing. Hans Peters
(Chairman of Institut Bauen und Umwelt e.V.)
Florian Pronold Dr. Matthew Fishwick,
(Managing Director Institut Bauen und Umwelt e.V.) (Independent verifier)
1 Environmental Product Declaration - Knauf Gips KG - Knauf Silentboard GKF
2. Product
Further information is available in the technical data sheet K717
2.1 Product description/Product definition Knauf Silentboard under www.knauf.com.
Knauf Silentboard GKF is a gypsum board with a high weight
per unit area and flexural ductility for enhanced sound Performance data of the product in accordance with the
insulation, consisting of a special gypsum core with a board declaration of performance with respect to its essential
liner cover. characteristics according to EN 520.
For the placing on the market of the product in the European 2.4 Delivery status
Union/European Free Trade Association (EU/EFTA) (with the Plasterboards Knauf Silentboard GKF according to DIN 18180
exception of Switzerland) Regulation (EU) No. 305/2011 (Type DFR according to EN 520) are delivered with a board
applies. The product Knauf Silentboard GKF needs a thickness of 12.5 mm as well as a size of 2500 or 2000 mm
declaration of performance taking into consideration EN 520 length, and 625 mm (width) with a half-rounded long edge
and the CE-marking. (HRAK) and front cut square edge (SK).
2.5 Base materials/Ancillary materials
For the application and use the respective national provisions
apply. Knauf Silentboard GFK consists of a special gypsum core (> 90
%), covered with a board liner (< 3 %), containing small
2.2 Application amounts (< 5 %) of starch, tensides, and fibre additives.
Knauf Silentboard GKF sound shield boards are used in all
interior fitting areas as cladding and for retrofitting drywalling This product contains substances listed in the candidate list
systems to fire protection standards and the high sound (23.01.2024) ECHA2024 exceeding 0.1 percentage by mass:
protection specifications. no.
Knauf Silentboard GKF are suitable for the following systems: This product contains other CMR substances in categories 1A
■ Metal stud partitions or 1B of Regulation (EC) No. 1272/2008 which are not on the
■ Furrings candidate list, exceeding 0.1 percentage by mass: no
■ Suspended ceilings
■ Room in a Room system Knauf Cubo Biocide products were added to this construction product or it
■ Upgrading of existing walls has been treated with biocide products (this then concerns a
treated product as defined by the (EU) Ordinance on Biocide
2.3 Technical Data Products No. 528/2012): no
The following technical data in condition on delivery is relevant
for the declared product: 2.6 Manufacture
Constructional data
The manufacturing process for gypsum boards is shown in
Name Value Unit
Figure 1.
Density acc. to DIN 18180 ≥ 1400 kg/m³
Thermal conductivity following EN 12664 0.26 W/(mK)
Water vapour resistance factor μ dry acc.
10 -
EN ISO 10456
Water vapour resistance factor μ wet acc.
4 -
EN ISO 10456
Shrinkage and expansion per 1 % change 0.005 -
mm/m
of relative air humidity - 0.008
Shrinkage and expansion per 1 Kelvin 0.013 -
mm/m
change of temperature - 0.02
Flexural breaking load longitudinal direction
≥ 725 N
acc. EN 520
Flexural breaking load transverse direction
≥ 300 N
acc. EN 520
2 Environmental Product Declaration - Knauf Gips KG - Knauf Silentboard GKF
Figure 1: Manufacturing process of gypsum boards free and dry conditions in a horizontal position.
The components of Knauf Silentboard GKF are suspended in Application
water and spread on a continuous sheet of board liner (visible During application, dust thresholds are to be observed
face, lower layer). Beforehand, the board liner is cut on the according to TRGS 900 and TRGS 559. The application and
sides for edge shaping. The slurry is covered with a second installation should follow the instruction sheets provided under
sheet of board liner (back surface) in the forming station and www.knauf.com, e.g., SIB01 Knauf Silentboard Systems.
the edges of the visible face board liner are flipped upwards.
On the subsequent board line the gypsum sets continuously Endless filament glass fibres are used in the manufacturing of
and is dried in a multi-level drier to the permitted residual Knauf Silentboard GKF for enhanced fire protection. These
moisture level. Drying is followed by the cutting of the boards to fibres do not fan out during application and therefore no fibre
the desired lengths. All processes within the company are dusts according to TRGS 521 occurs.
certified according to ISO 9001.
2.9 Packaging
2.7 Environment and health during manufacturing Plasterboards Knauf Silentboard GKF are stacked on reusable
The production of Knauf Silentboard GKF is subject to the pallets and protected with a polyethylene (PE) film.
German emission control regulations BImSchG. Greenhouse
gas emissions are measured due to CO emissions trading. 2.10 Condition of use
2
Knauf Silentboard sound shield boards are used in all interior
The German manufacturing sites for the production of Knauf
fitting areas as cladding and for retrofitting drywalling systems
Silentboard GKF are certified according to ISO 50001 as well
to fire protection standards and the highest sound protection
as certified with the occupational safety standard 'Sicher mit
specifications. There is no alteration of the material composition
System' (Systematic Safety) from the German trade association
during use.
BG RCI.
2.11 Environment and health during use
Gypsum from the flue-gas desulphurization plants of coal-fired
High sound protection performance is especially provided in the
power stations is used in addition to natural gypsum.
low frequency range. By this, Knauf Silentboard GKF
Production waste as well as dust from the filtration plants are
contributes to health protection and enhanced comfort inside
recycled internally and fed back into the production of
buildings.
plasterboards.
2.8 Product processing/Installation According to the emission test of Eurofins Product Testing A/S
(Eurofins2021), no hazardous substances are emitted above
Storage
permissible thresholds during use.
Knauf Silentboard GKF should be stored indoors under dust-
3 Environmental Product Declaration - Knauf Gips KG - Knauf Silentboard GKF
2.12 Reference service life 2.14 Re-use phase
There was no reference service life determined according to Re-use
ISO 15686-1. However, a service life of 50 years can be Once plasterboards Knauf Silentboard GKF are installed, they
considered for gypsum plasterboards according to the are not suited for re-use in an unchanged way. Prior to
Guideline for Sustainable Building BBSR2017. There are no collection, Knauf Silentboard GKF should be separated from
influences on the ageing of Knauf Silentboard GKF during use other used building materials and pruned of foreign matter, e.g.,
when following the established engineering practice. metals from the substructure already on site for easier recycling
or disposal.
2.13 Extraordinary effects
Fire Further use
The reaction to fire of Knauf Silentboard GKF is classified as Residual materials from new plasterboards Knauf Silentboard
follows according to EN 520 in conjunction with EN 13501-1. GKF, e.g., from cut waste at the building site, can be disposed
Fire protection of at a landfill.
Name Value
Recycling
Building material class; fire behaviour class A2
In principle, gypsum boards can be recycled by standard
Smoke gas development; smoke production s1 recycling processes. However, Knauf Silentboard GKF is
Burning droplets; flaming droplets/particles d0 currently not suited for recycling.
A2 = non-combustible 2.15 Disposal
s1 = no smoke
Plasterboards Knauf Silentboard GKF have to be disposed of in
d0 = no burning fall-off/drop-off
compliance with the following waste codes of the European
Waste Catalogue:
Water
17 08 02 - gypsum-based construction materials other than
Knauf Silentboard GKF show a small tendency to swell or
those mentioned in 17 08 01
shrink within changes of the climatic conditions. However, a
17 09 04 - mixed construction and demolition wastes other than
permanent exposure to wet conditions or very high levels of
those mentioned in 17 09 01, 17 09 02 and 17 09 03
relative humidity may lead to a decrease in strength. An
instruction sheet about restoration of flood damage is available
National disposal guidelines have to be observed. In Germany,
under www.knauf.com BSDH2013.
Knauf Silentboard GKF are to be disposed of at landfills of
landfill category 1 or higher according to the regulation of
landfills DepV.
Mechanical destruction
Minor damages on plasterboards Knauf Silentboard GKF can 2.16 Further information
be mended with suitable gypsum based filling materials. The Further information about Knauf Silentboard GKF, e.g., the
installation with screws allows an easy exchange of heavily technical data sheet or the product safety information sheet are
damaged boards. In this case, the substructure should available at www.knauf.com.
be examined, too, and replaced if necessary.
3. LCA: Calculation rules
• disassembly (C1)
3.1 Declared Unit • transport to recycling facility or landfill site (C2)
The declared unit is 1 m² of Knauf Silentboard GKF with a • landfilling at end of life (C4)
thickness of 12.5 mm, weight of approx. 17.5 kg/m². • credits in D from incineration with energy recovery of
Declared unit packaging material in A5
Name Value Unit
The life cycle of Knauf Silentboard GKF is outlined in Figure 2.
Declared unit 1 m2
Conversion factor to 1 kg 0.057 m²/kg
Grammage 17.5 kg/m2
Layer thickness 0.0125 m
3.2 System boundary
The EPD is a declaration cradle to gate with options, modules
C1–C4, and module D (A1–A3, C, D, and additional modules
A4 and A5).
This Environmental Product Declaration according to EN 15804
contains:
• provision of raw materials and transport to plant,
production of boards (A1-A3) including thermal energy
for calcination and drying (from natural gas, geographic
scope: DE), as well as electricity (residual mix DE) •
transport to building site (A4)
• installation at building site (A5) including the incineration Figure 2: Principal life cycle of gypsum boards
of transport packaging
3.3 Estimates and assumptions
4 Environmental Product Declaration - Knauf Gips KG - Knauf Silentboard GKF
Some raw material and additives were not available in the datasets from Sphera's Managed LCA content database,
background database and therefore were either substituted exclusively. The used background data sets are no older than 5
with similar material or modelled with own processes. years. Due to the substitution of materials which had to be
considered in the LCA modelling, the overall data quality was
For transport, a general payload of 50 % is assumed. Transport evaluated as satisfactory.
to the building site (module A4) as well as transport from the
building site to the collecting site or landfill (module C2) is 3.7 Period under review
calculated with a standard distance of 100 km. These are not The modelling is based on the annual production of Knauf
actual transport distances but shall facilitate the extrapolation to Silentboard GKF in production year 2022.
the 'real' distances on building level.
3.8 Geographic Representativeness
3.4 Cut-off criteria Land or region, in which the declared product system is
All raw materials for the manufacturing of plasterboards Knauf manufactured, used or handled at the end of the product´s
Silentboard GKF, the required energy, water and the resulting lifespan: Global
emissions are considered in the life cycle assessment. That
way, recipe components with a share even smaller than 1 %
3.9 Allocation
are included. All neglected processes contribute less than 5 %
Allocations are avoided in the modelling. Energy consumptions
to the total mass or less than 5 % to the total energy
of different board types are monitored product specific.
consumption.
Therefore, no co-product allocation was required. Beyond that,
3.5 Background data allocations are only applied in the background data.
For modelling, the software LCA for Experts version 10.7.1.28
3.10 Comparability
with the Managed LCA content version 2023.2 from Sphera
Basically, a comparison or an evaluation of EPD data is only
was used. Data sets for Germany were used for the life cycle
possible if all the data sets to be compared were created
inventory as much as possible, especially for the provision of
according to EN 15804 and the building context, respectively
electricity and thermal energy.
the product-specific characteristics of performance, are taken
3.6 Data quality into account.
The LCA of Knauf Silentboard GKF was modelled by using
4. LCA: Scenarios and additional technical information
countries.
Characteristic product properties of biogenic carbon
Manufacturing (A3)
Biogenic carbon in product and packaging per 1 m² board Natural gypsum and gypsum from the flue-gas desulphurization
according to EN 15804+A2 is calcinated prior to the mixing with other components. FGD
gypsum is usually delivered as damp material and, thus, must
Name ValueUnit
be dried before calcination. Stucco, mineral fillers and additives
kg
Biogenic carbon content in product 0.221 are mixed with water and processed as described in section
C
2.6. The addition of water allows the incorporation of water of
Biogenic carbon content in accompanying kg crystallization into the crystal lattice of calcium sulphate, i.e.,
0.042
packaging C gypsum becomes settled and hardened. Redundant surface
water is removed in a multi-level dryer.
Note: 1 kg of biogenic carbon is equivalent to 44/12 kg of CO .
2
Transport to building site (A4)
Product Stage (A1-A3) For transport, a standard distance of 100 km by truck is
assumed. This declaration facilitates the extrapolation of the
Supply of raw materials (A1) results in A4 to the real distance.
Knauf Silentboard GKF consists of a gypsum core and barytes
Name Value Unit
which is reinforced with mineral fillers and covered with board
Transport distance 100 km
liner. The natural gypsum is mainly extracted from open-cast
Capacity utilisation (including empty runs) 50 %
mining in close vicinity to the manufacturing site. Furthermore,
gypsum from the flue-gas desulphurization of coal-fired power Gross density of products transported 1400 kg/m3
stations (FGD gypsum) is used as a raw material. Board liner
for the covering of gypsum core is produced from recycled Assembly at building site (A5)
waste paper which is certified by FSC and/or PEFC. Additives The installation in the building includes the electricity
are added for an easier processing and a fine adjustment of consumption for fastening the Knauf Silentboard GKF.
properties of plasterboards Knauf Silentboard GKF. These Accessories such as screws or the substructure itself are not
additives add up to less than 5 %. part of the LCA in this EPD. The energy consumption for the
electrical devices was considered with 0.0018 kWh/m².
Transport of raw materials(A2)
Natural gypsum is extracted from mines close to the The waste material (0.892 kg/m²) from the construction site is
manufacturing sites of Knauf Silentboard GKF. Accordingly, transported by truck to a landfill and disposed of. The
transport distances are short and trucks can be used. FGD replacement of this construction waste is considered in A5 as
gypsum is transported by rail from coal-fired power plants. The well.
heavy spar is produced predominantly in Germany and also
delivered by truck. Baryte can also be delivered from overseas The packaging material, re-usable wooden pallets and PE-film,
by container ship. Further raw materials are supplied by truck is incinerated. The credits from this process are reported in
from manufacturers within Germany or from neighbouring Module D.
5 Environmental Product Declaration - Knauf Gips KG - Knauf Silentboard GKF
Currently, Knauf Silentboard GKF is not recycled. Therefore,
Name Value Unit module C3 is declared with 0 impacts.
Electricity consumption 0.0018 kWh
Disposal (C4) includes the disposal of 100 % Knauf Silentboard
Material loss 0.892 kg
GKF at inert landfill.
Use phase (B1-B7) Disposal (C4)
Excluded since no environmental impacts/benefits are
Name Value Unit
expected. A service life of 50 years can be considered for
Collected separately 17.5 kg
gypsum plasterboards according to the Guideline for
Sustainable Building BBSR2017. Collected as mixed construction waste - kg
Reuse - kg
End of life (C1-A4) Recycling - kg
The demolition (C1) of the Knauf Silentboard GKF from the
Energy recovery - kg
building is considered to be done 100 % manually. It was
Landfilling 17.5 kg
assumed that the deconstruction would take place without
further processing of the waste.
Reuse-, recover- and recycling potential (D)
Module D contains only credits for exported energy from
For the transport (C2) from the demolition site to the landfill by
incineration of packaging material (results only from A5).
truck, a distance of 100 km was assumed in the calculation.
Name Value Unit
Transport (C2)
Incineration of the packaging material 100 %
Name Value Unit
Transport distance 100 km
Capacity utilisation (including empty runs) 50 %
6 Environmental Product Declaration - Knauf Gips KG - Knauf Silentboard GKF
5. LCA: Results
DESCRIPTION OF THE SYSTEM BOUNDARY (X = INCLUDED IN LCA; MND = MODULE OR INDICATOR NOT DECLARED; MNR
= MODULE NOT RELEVANT)
Benefits and
Construction loads beyond
Product stage Use stage End of life stage
process stage the system
boundaries
la ire ta m w a Ry lp p u s tro p s n a rT g n iru tc a fu n a M e h t m o rf tro p s n a rTe tis e h t o t e ta g y lb m e s s A e s U e c n a n e tn ia M ria p e R tn e m e c a lp e R tn e m h s ib ru fe R y g re n e la n o ita re p Oe s u re ta w la n o ita re p Oe s u n o itc u rts n o c -e Dn o itilo m e d tro p s n a rT g n is s e c o rp e ts a W la s o p s iD -e s u e R-y re v o c e R-g n ilc y c e Rla itn e to p
A1 A2 A3 A4 A5 B1 B2 B3 B4 B5 B6 B7 C1 C2 C3 C4 D
X X X X X MND MND MNR MNR MNR MND MND X X X X X
RESULTS OF THE LCA - ENVIRONMENTAL IMPACT according to EN 15804+A2: 1 m² Knauf Silentboard GKF 12.5 mm; approx.
17.5 kg/m²
Parameter Unit A1-A3 A4 A5 C1 C2 C3 C4 D
GWP-total kg CO 2 eq 1.4E+00 1.5E-01 3.2E-01 0 1.5E-01 0 1.06E+00 -5.45E-02
GWP-fossil kg CO 2 eq 2.36E+00 1.46E-01 1.61E-01 0 1.46E-01 0 2.64E-01 -5.42E-02
GWP-biogenic kg CO 2 eq -9.54E-01 2.12E-03 1.58E-01 0 2.12E-03 0 7.94E-01 -2.48E-04
GWP-luluc kg CO 2 eq 2.84E-03 1.36E-03 3.22E-04 0 1.36E-03 0 8.32E-04 -3.54E-06
ODP kg CFC11 eq 1.77E-11 2.3E-14 9.51E-13 0 2.3E-14 0 6.89E-13 -4.27E-13
AP mol H+ eq 4.37E-03 1.93E-04 3.64E-04 0 1.93E-04 0 1.9E-03 -6.79E-05
EP-freshwater kg P eq 1.76E-05 5.38E-07 9.71E-07 0 5.38E-07 0 5.41E-07 -8.81E-08
EP-marine kg N eq 1.39E-03 6.77E-05 1.1E-04 0 6.77E-05 0 4.91E-04 -1.99E-05
EP-terrestrial mol N eq 1.41E-02 7.94E-04 1.18E-03 0 7.94E-04 0 5.4E-03 -2.13E-04
kg NMVOC
POCP 3.36E-03 1.67E-04 2.83E-04 0 1.67E-04 0 1.48E-03 -5.53E-05
eq
ADPE kg Sb eq 2.1E-07 9.87E-09 1.24E-08 0 9.87E-09 0 1.24E-08 -3.9E-09
ADPF MJ 3.84E+01 2.02E+00 2.36E+00 0 2.02E+00 0 3.57E+00 -1E+00
m3 world eq
WDP 6.98E-02 1.84E-03 2.5E-02 0 1.84E-03 0 2.93E-02 -5.18E-03
deprived
GWP = Global warming potential; ODP = Depletion potential of the stratospheric ozone layer; AP = Acidification potential of land and water; EP =
Eutrophication potential; POCP = Formation potential of tropospheric ozone photochemical oxidants; ADPE = Abiotic depletion potential for non-fossil
resources; ADPF = Abiotic depletion potential for fossil resources; WDP = Water (user) deprivation potential)
RESULTS OF THE LCA - INDICATORS TO DESCRIBE RESOURCE USE according to EN 15804+A2: 1 m² Knauf Silentboard
GKF 12.5 mm; approx. 17.5 kg/m²
Parameter Unit A1-A3 A4 A5 C1 C2 C3 C4 D
PERE MJ 1.05E+01 1.47E-01 2.53E+00 0 1.47E-01 0 5.84E-01 -2.92E-01
PERM MJ 7.71E+00 0 -1.55E+00 0 0 0 0 0
PERT MJ 1.82E+01 1.47E-01 9.73E-01 0 1.47E-01 0 5.84E-01 -2.92E-01
PENRE MJ 3.81E+01 2.03E+00 2.57E+00 0 2.03E+00 0 3.57E+00 -1E+00
PENRM MJ 2.97E-01 0 -2.1E-01 0 0 0 0 0
PENRT MJ 3.84E+01 2.03E+00 2.36E+00 0 2.03E+00 0 3.57E+00 -1E+00
SM kg 3.59E-01 0 0 0 0 0 0 0
RSF MJ 0 0 0 0 0 0 0 0
NRSF MJ 0 0 0 0 0 0 0 0
FW m3 1.32E-02 1.64E-04 1.19E-03 0 1.64E-04 0 9E-04 -2.36E-04
PERE = Use of renewable primary energy excluding renewable primary energy resources used as raw materials; PERM = Use of renewable primary
energy resources used as raw materials; PERT = Total use of renewable primary energy resources; PENRE = Use of non-renewable primary energy
excluding non-renewable primary energy resources used as raw materials; PENRM = Use of non-renewable primary energy resources used as raw
materials; PENRT = Total use of non-renewable primary energy resources; SM = Use of secondary material; RSF = Use of renewable secondary fuels;
NRSF = Use of non-renewable secondary fuels; FW = Use of net fresh water
RESULTS OF THE LCA – WASTE CATEGORIES AND OUTPUT FLOWS according to EN 15804+A2:
1 m² Knauf Silentboard GKF 12.5 mm; approx. 17.5 kg/m²
Parameter Unit A1-A3 A4 A5 C1 C2 C3 C4 D
HWD kg 3.5E-09 1.04E-11 1.8E-10 0 1.04E-11 0 7.69E-11 -5.32E-11
NHWD kg 5.1E-01 3.13E-04 9.23E-01 0 3.13E-04 0 1.79E+01 -4.95E-04
RWD kg 9.29E-04 3.96E-06 5.34E-05 0 3.96E-06 0 4.01E-05 -7.74E-05
CRU kg 0 0 0 0 0 0 0 0
MFR kg 0 0 0 0 0 0 0 0
MER kg 0 0 0 0 0 0 0 0
EEE MJ 0 0 2.58E-01 0 0 0 0 0
7 Environmental Product Declaration - Knauf Gips KG - Knauf Silentboard GKF
EET MJ 0 0 4.64E-01 0 0 0 0 0
HWD = Hazardous waste disposed; NHWD = Non-hazardous waste disposed; RWD = Radioactive waste disposed; CRU = Components for re-use;
MFR = Materials for recycling; MER = Materials for energy recovery; EEE = Exported electrical energy; EET = Exported thermal energy
RESULTS OF THE LCA – additional impact categories according to EN 15804+A2-optional:
1 m² Knauf Silentboard GKF 12.5 mm; approx. 17.5 kg/m²
Parameter Unit A1-A3 A4 A5 C1 C2 C3 C4 D
Disease
PM 2.15E-07 1.41E-09 1.23E-08 0 1.41E-09 0 2.34E-08 -5.76E-10
incidence
IR kBq U235 eq 1E-01 5.81E-04 6.04E-03 0 5.81E-04 0 4.56E-03 -1.29E-02
ETP-fw CTUe 9.79E+00 1.44E+00 7.56E-01 0 1.44E+00 0 1.93E+00 -1.4E-01
HTP-c CTUh 5.69E-10 2.92E-11 4.86E-11 0 2.92E-11 0 3E-10 -1.11E-11
HTP-nc CTUh 3.37E-08 1.3E-09 3.52E-09 0 1.3E-09 0 3.16E-08 -2.73E-10
SQP SQP 3.74E+01 8.37E-01 2.02E+00 0 8.37E-01 0 9E-01 -1.92E-01
PM = Potential incidence of disease due to PM emissions; IR = Potential Human exposure efficiency relative to U235; ETP-fw = Potential comparative
Toxic Unit for ecosystems; HTP-c = Potential comparative Toxic Unit for humans (cancerogenic); HTP-nc = Potential comparative Toxic Unit for humans
(not cancerogenic); SQP = Potential soil quality index
Disclaimer 1 – for the indicator “Potential Human exposure efficiency relative to U235”. This impact category deals mainly with the
eventual impact of low dose ionizing radiation on human health of the nuclear fuel cycle. It does not consider effects due to possible
nuclear accidents, occupational exposure nor due to radioactive waste disposal in underground facilities. Potential ionizing radiation
from the soil, from radon and from some construction materials is also not measured by this indicator.
Disclaimer 2 – for the indicators “abiotic depletion potential for non-fossil resources”, “abiotic depletion potential for fossil resources”,
“water (user) deprivation potential, deprivation-weighted water consumption”, “potential comparative toxic unit for ecosystems”,
“potential comparative toxic unit for humans – cancerogenic”, “Potential comparative toxic unit for humans - not cancerogenic”,
“potential soil quality index”. The results of this environmental impact indicator shall be used with care as the uncertainties on these
results are high or as there is limited experienced with the indicator.
6. LCA: Interpretation
In general, the highest environmental impacts of Knauf C4 contributes also considerably to the impact categories
Silentboard GKF result from the product stage A1-A3 with the Water deprivation potential WDP (24 %), Eutrophication –
exception of non-hazardous waste disposed NHWD. For this marine EP-m (23 %), Eutrophication – terrestrial (25 %),
indicator, module C4 and the disposal of the boards at inert Photochemical ozone depletion potential POCP (27 %),
landfill leads to the highest overall contribution. Acidification potential AP (27 %), Human toxicity - cancer
In modules A1-A3, major contributions result from the provision effects HTP-c (31 %), and Human toxicity – non-cancer effects
of raw materials to the overall life cycle impacts of the product. HTP-nc (44 %).
Exceptions are Hazardous waste disposed HWD (approx. 9 %),
Non-hazardous waste disposed NHWD (< 1 %), Potential soil Transports in A4 and in C2 cause only minor contributions to
quality index SQP (approx. 27 %), and Global Warming the overall life cycle impacts, due to assumed distances of 100
Potential land use and land use change GWP-luluc (approx. 14 km in both modules. Exceptions are Ecotoxicity, freshwater
%). ETP-fw (approx. 9 %) and the Global Warming Potential land
use and land use change GWP-luluc (approx. 20 %).
The non-hazardous waste disposed NHWD, is dominated by
the disposal C4 by almost 92 %. This was expected since there Some small credits given in module D result from the
is no recycling at end of life but a complete landfilling. The high incineration and recycling of packaging only. The disassembled
contribution of C4 to GWP-t results from the emission of product is landfilled after disassembly.
biogenic carbon incorporated in the plasterboard. Landfilling in
7. Requisite evidence
Test after 3 days (limit value)
7.1 Leaching (sulphates and heavy metals)
Name Value Unit
Plasterboards Knauf Silentboard GKF show a leaching
behaviour typical for gypsum-based building products Dre2006. TVOC < 10 mg/m²
That is why disposal is only allowed in landfills from landfill Total carcinogens < 0.01 mg/m²
category 1 in Germany DepV2021.
Plasterboards Knauf Silentboard GKF are classified in water Test after 28 days (limit value)
hazard class 1 (slightly water-hazardous) AwSV. Name Value Unit
TVOC < 1.0 mg/m³
7.2 Radioactivity
TSVOC < 0.1 mg/m³
According to Geh2012 and RP 112 dose values and radon
R (dimensionless) < 1 -
concentrations of gypsum-based building products are below
0.3 mSv/a. Thus, they can be used without restrictions. Sum of VOC without NIK/LCI < 0.1 mg/m³
Formaldehyde < 0.1 mg/m³
7.3 VOC emissions Total carcinogens < 0.001 mg/m³
According to the emission test from Eurofins Product Testing
VOC emission tests showed that Knauf Silentboard GKF
A/S, no hazardous substances are emitted above permissible
significantly undercut the required thresholds.
thresholds during use Eurofins2021.
8 Environmental Product Declaration - Knauf Gips KG - Knauf Silentboard GKF
8. References
Standards 2015-08-31 (BGBI. I p. 1474)
DIN 18180 DepV
DIN 18180:2014-09, Gypsum plasterboards - Types and Verordnung über Deponien und Langzeitlager
requirements (Deponieverordnung – DepV), German landfill ordinance, last
amended and supplemented: 2021-07-09
EN 520
EN 520:2009-12, Gypsum plasterboards - Definitions, ECHA
requirements and test methods European Chemicals Agency (ECHA), Candidate List of
Substances of Very High Concern for Authorisation (published
EN 12664 in accordance with Article 59(10) of the REACH Regulation),
DIN EN 12664: Thermal Performance of Building Materials and http://echa.europa.eu/de/candidate-list- table, Revision: 2024-
Products - Determination of Thermal Resistance by Means of 01-23
Guarded Hot Plate and Heat Flow Meter Methods - Dry and
Moist Products with Medium and Low Thermal European Waste Code
Guidance on classification of waste according to EWC-Stat
EN 13501-1 categories, Supplement to the Manual for the Implementation of
Fire classification of construction products and building the Regulation (EC) No 2150/2002 on Waste Statistics,
elements – Part 1: Classification using data from reaction to fire COMMISSION OF THE EUROPEAN
tests; German version EN 13501-1:2018 COMMUNITIES/EUROSTAT, v2, December 2010
EN 15804 Regulation (EU) No 305/2011
EN 15804:2012+A2:2019+AC:2021, Sustainability of Regulation (EU) No 305/2011 of the European Parliament and
construction works — Environmental Product Declarations — of the Council of 9 March 2011 laying down harmonized
Core rules for the product category of construction products. conditions for the marketing of construction products
ISO 9001 Regulation (EC) No 528/2012
DIN EN ISO 9001:2015-09; Quality management system – Regulation (EU) No 528/2012 of the European Parliament and
Requirements of the Council of 22 May 2012 concerning the making available
on the market and use of biocidal products
ISO 10456
EN ISO 10456-1:2010-05: Building materials and products - Regulation (EC) No. 1272/2008
Hygrothermal properties – Tabulated design values and Regulation (EC) No 1272/2008 of the European Parliament and
procedures for determining declared and design thermal of the Council of 16 December 2008 on classification, labelling
values - Technical Corrigendum 1 (ISO 10456:2007/Cor and packaging of substances and mixtures
1:2009)
TRGS 521
ISO 11885 Technical Rules for Hazardous Substances No. 521:
EN ISO 11885:2009, Water quality – Determination of selected 'Demolition, reconstruction and maintenance work with
elements by inductively coupled plasma optical emission biopersistent mineral wools', German Federal Institute for
spectrometry (ICP-OES) Occupational Safety and Health, 2008-02
ISO 14025 TRGS 559
EN ISO 14025:2011, Environmental labels and declarations — Technical Rules for Hazardous Substances No. 559: 'Mineral
Type III environmental declarations — Principles and Dust', German Federal Institute for Occupational Safety and
procedures. Health, 2010-02
ISO 15686-1 TRGS 900
ISO 15686-1:2011: Buildings and constructed assets -- Service Technical Rules for Hazardous Substances No. 900:
life planning -- Part 1: General principles and framework 'Arbeitsplatzgrenzwerte' (Occupational Exposure Limit Values,
OELS), German Federal Institute for Occupational Safety and
ISO 50001 Health, 2024-01
EN ISO 50001:2018, Energy management systems –
Requirements with guidance for use
Further References
Regulations
BBSR2017
AwSV Service life of building components for life cycle analyses acc.
Verordnung über Anlagen zum Umgang mit to the Sustainable Building Assessment System (BNB) --
wassergefährdenden Stoffen 1,2 (AwSV) 18.04.2017 vom Nutzungsdauer von Bauteilen für Lebens-zyklusanalysen nach
Bundesministerium der Justiz Bewertungssystem Nachhaltiges Bauen (BNB) 2017-02-24 vom
Bundesinstitut für Bau-, Stadt-, Raumforschung (BBSR)
BImSchG
Act on the Prevention of Harmful Effects on the Environment BDSH2013
Caused by Air Pollution, Noise, Vibration and Similar Bauschäden durch Hochwasser – Tipps für die Sanierung
Phenomena (Federal Immission Control Act - BImSchG), (Flood damage - tips for recovery), instruction sheet, Knauf
Publication 2013-05-2017 (BGBI. I p. 1274), last amended Gips KG (editor), Iphofen, 2013, www.knauf.de
9 Environmental Product Declaration - Knauf Gips KG - Knauf Silentboard GKF
BG RCI IBU PCR Part A
Occupational health and safety management: Systematic Institut Bauen und Umwelt e.V.: Product Category Rules for
Safety, editor: The German Social Accident Insurance Building-Related Products and Services Part A: Calculation
Institution for the Raw Materials and Chemical Industry, Rules for the Life Cycle Assessment and Requirements on the
Heidelberg, 2021-12-01 Project Report according to EN 15804+A2:2019, v1.1.2, 2021-
09-02
Dre2006
H. Drexler, Test report no. 1080556 AU-23572, Dorfner IBU PCR Part B "Plasterboards"
Analysenzentrum und Anlagenplanungsgesellschaft mbH, Institut Bauen und Umwelt e.V.: PCR Guidance-Texts for
Hirschau, 11.01.2006 (originator: Bundesverband Gips e. V., Dr. Building-Related Products and Services Part B: Requirements
H.-J. Kersten, Berlin) on the EPD for Plasterboard, v5, 2023-07-11
Eurofins2021 LCA for Experts (GaBi)
VOC Emission Test Report for Knauf Silentboard GKF 12.5 mm LCA for Experts (v10.7.1.28): Software-System and Databases
by the institute 'Eurofins Product Testing A/S in Galten- for Life Cycle Engineering, Sphera Solutions GmbH,
Denmark; 2021-10-29 Leinfelden- Echterdingen, Germany, 2023 (database version
2023.2)
Geh2012
K. Gehrcke, B. Hoffmann, U. Schkade, V. Schmidt, K. Managed LCA content
Wichterey: Natürliche Radioaktivität in Baumaterialien und die Managed LCA content (database), Sphera Solutions GmbH,
daraus resultierende Strahlenexposition, Report BfS-SW-14/12, Content version 2023.2
Bundesamt für Strahlenschutz (editor), http://nbn-
resolving.de/urn:nbn:de:0221-201210099810, Salzgitter, 2012
Technical brochures Knauf
Gips-DB Downloadable under www.knauf.com
Gips-Datenbuch, editor: Bundesverband Gips e. V. (German
association of gypsum manufacturers), Berlin, 2013 K717
K717.de_ENG Silentboard GKF technical data sheet, 2023-04
IBU 2022
Institut Bauen und Umwelt e.V.: General Instructions for the SIB01
EPD programme of Institut Bauen und Umwelt e.V., Version SIB01.de_ENG Knauf Silentbaord Systems Sound Insulation
2.1, Berlin: Institut Bauen und Umwelt e.V., 2022; www.ibu- with Premium Drywalling, technical brochure, 2018-01
epd.com
10 Environmental Product Declaration - Knauf Gips KG - Knauf Silentboard GKF
Publisher
Institut Bauen und Umwelt e.V. +49 (0)30 3087748- 0
Hegelplatz 1 info@ibu-epd.com
10117 Berlin www.ibu-epd.com
Germany
Programme holder
Institut Bauen und Umwelt e.V. +49 (0)30 3087748- 0
Hegelplatz 1 info@ibu-epd.com
10117 Berlin www.ibu-epd.com
Germany
Author of the Life Cycle Assessment
Knauf Gips KG 0049 9001 31-1000 *
Am Bahnhof 7 knauf-direkt@knauf.de
97346 Iphofen www.knauf.de
Germany
Owner of the Declaration
Knauf Gips KG 0049 9001 31-1000 *
Am Bahnhof 7 knauf-direkt@knauf.com
97346 Iphofen www.knauf.com
Germany
11 Environmental Product Declaration - Knauf Gips KG - Knauf Silentboard GKF
