ENVIRONMENTAL PRODUCT DECLARATION
as per ISO 14025 and EN 15804+A2
Owner of the Declaration ONDULINE SA
Publisher Institut Bauen und Umwelt e.V. (IBU)
Programme holder Institut Bauen und Umwelt e.V. (IBU)
Declaration number EPD-OND-20230362-ICD2-EN
Issue date 22.03.2024
Valid to 21.03.2029
Corrugated bitumen sheets for under-roofing application
ONDULINE SA
www.ibu-epd.com | https://epd-online.com
1. General Information
ONDULINE SA Corrugated bitumen sheets for under-roofing
application
Programme holder Owner of the declaration
IBU – Institut Bauen und Umwelt e.V. ONDULINE SA
Hegelplatz 1 Quai Gallieni 24
10117 Berlin 92150 SURESNES
Germany France
Declaration number Declared product / declared unit
EPD-OND-20230362-ICD2-EN 1m² corrugated bitumen sheets for under-roofing application
This declaration is based on the product category rules: Scope:
Corrugated bitumen materials for roofing and external wall This Life Cycle Assessment study is relevant for corrugated bitumen
cladding, 01.08.2021 sheets produced in the manufacturing plants of Onduline-SA located in
(PCR checked and approved by the SVR) Malaysia, Poland, Spain and Turkey. This EPD represents an average
EPD, where a weighted average product (with an average grammage of
2.93 kg/m²) is formed based on data provided by the above-mentioned
Issue date plants. In this study, the data collected refer to the years 2020 to 2022.
The owner of the declaration shall be liable for the underlying information
22.03.2024
and evidence; the IBU shall not be liable with respect to manufacturer
information, life cycle assessment data and evidences.
Valid to
The EPD was created according to the specifications of EN 15804+A2. In
21.03.2029 the following, the standard will be simplified as EN 15804.
Verification
The standard EN 15804 serves as the core PCR
Independent verification of the declaration and data according to ISO
14025:2011
internally X externally
Dipl.-Ing. Hans Peters
(Chairman of Institut Bauen und Umwelt e.V.)
Florian Pronold Dr.-Ing. Nikolay Minkov,
(Managing Director Institut Bauen und Umwelt e.V.) (Independent verifier)
1 Environmental Product Declaration - ONDULINE SA - Corrugated bitumen sheets for under-roofing application
2. Product
2.1 Product description/Product definition 2.2 Application
The products covered by this EPD are corrugated bitumen Corrugated bitumen sheet's main function is to provide water
sheets, which are made from cellulose fibres and bitumen. tightness on pitched roofs and walls. They can be applied on
Bitumen is used to give the products their waterproofing wooden or metallic battens and purlins but also on full decks.
properties. Corrugated bitumen sheets can be produced in a The type of substructure has to be chosen according to the
variety of sizes and colours. These products are intended for shape of the roof. They should be laid onto the substructure
under-roofing applications. staggered and overlapped. They can be combined with several
insulation systems.
The sales-weighted average weight of finished sheets is 2.93kg
per m². 2.3 Technical Data
Onduline SA's corrugated bitumen sheets are produced and
The list of product codes and trade names covered by this EPD delivered according to the requirements of the standard EN
is detailed below: 14964.
MALAYSIA: For further details, see Technical Data Sheets at
- S05004 ONDULINE T50H Black http://www.onduline.com.
- S05026 ONDULINE T940H RED Red Tile Constructional data
- S05028 T50H DR RED 29 Red Tile
Name Value Unit
POLAND:
Length 1820 - 2000 mm
- S06011 ONDULINE T220 Autumn Red
- S06013 WL T220 UL Asphalt Width 864 - 1056 mm
- S06014 ONDULINE T190 Autumn Red Thickness 2.1 - 2.9 mm
- S06015 WL T190 L Black Grammage 2.41 - 3.39 kg/m2
- S06018 ONDULINE T95 Autumn Red
- S06025 WL T95 Black Performance data of the product in accordance with the
- S06029 ONDULINE T220 DRP Ocher declaration of performance with respect to its essential
- S06037 G95 ECO 10 SR-110 (UR) Black characteristics according to EN 14964, October 2006 – Rigid
SPAIN: underlays for discontinuous roofing – type OL.
- S08013 ONDULINE T235 Autumn Red
2.4 Delivery status
- S08015 WL T235 UL Asphalt
Onduline Corrugated Bitumen Sheets are delivered on pallets
- S08016 ONDULINE T380 Autumn Red
only. They are packaged by 100 or 150 or 300 or 420 sheets
- S08017 ONDULINE T470 Autumn Red
per pallets.
- S08018 WL T50 UL Asphalt
- S08019 ONDULINE T50 Autumn Red - ISOLINE LOW LINE
2.5 Base materials/Ancillary materials
- S08024 ONDULINE T940 Autumn Red
The product components are waste paper/cardboard, bitumen,
- S08030 ONDULINE T95 Autumn Red
resin, pigment, binder, paint loads, drainage agent, antifoaming
- S08036 ONDULINE T235 DRP Silver Grey
agent/defoamer, dispersing agent, biocide and pH regulator.
- S08036 ONDULINE T235 DRP Ocher
- S08036 ONDULINE T235 DRP Terracotta Name Value Unit
- S08037 WL T235 Brown Waste paper, cardboard (post-consumer
50 %
- S08037 WL T235 Autumn Red recycled material content)
- S08038 WL T235 SRP Ocher Bitumen 48 %
- S08038 WL T235 SRP Terracotta
Resin 0.9 %
- S08039 ONDULINE T95 DRP Ocher
approx.
- S08043 WL T95 Black SPAIN Others %
1.1
- S08049 T50G Black
- S08050 ONDULINE T940H Values presented in the table are for the average product
- S08052 ONDULINE T50H Black declared in this EPD.The sales-weighted average weight of
TURKEY: finished sheets is 2.93kg per m².
- S09020 ONDULINE T50M Black
- S09036 ONDULINE T190 L26 (RUFOLINE) Black The products covered by this EPD do not contain substances
- S09038 ONDULINE T50H Black listed in the 'Candidate List of Substances of Very High
- S09042 ONDULINE T95 Red Concern for Authorisation' (date: 14/06/2023) exceeding 0.1
- S09043 ONDULINE T50H FR percentage by mass. These construction products are not a
- S09044 T50H DR RED 26 Red 130 substance or mixture under the chemical law (REACH).
- S09047 ONDULINE T430H
- S09055 T50H DR RED 29 SE Red 130 The products covered by this EPD do not contain other CMR
- S09057 T50H DR RED 29 Red 130 substances in categories 1A or 1B which are not on the
- S09061 ONDULINE T50M CT candidate list, exceeding 0.1 percentage by mass.
For the placing on the market of the product in the European Coating additives have been added and remain on the
Union/European Free Trade Association (EU/EFTA) (with the references covered by this EPD:
exception of Switzerland) Regulation (EU) No. 305/2011 (CPR)
• Octylisothiazolinone (OIT), biocide (CAS number:
applies. The corrugated bitumen sheets need a declaration of
26530-20-1),
performance taking into consideration EN 14964, October 2006
• Terbutryn, biocide (CAS number: 886-50-0),
– Rigid underlays for discontinuous roofing – type OL –
• Zinc pyrithione, biocide (CAS number: 13463-41-7),
Definitions and characteristics and the CE marking.
2 Environmental Product Declaration - ONDULINE SA - Corrugated bitumen sheets for under-roofing application
• Polyethylenimine, hydrophobic agent (CAS number: that the roof is watertight. These overlaps mean that more than
9002-98-6). 1sqm of sheet is needed to properly cover 1sqm of roof, which
Octylisothiazolinone (2-octyl-isothiazol-3(2H)-one) is a chemical is what we call "overlapping losses". See below for ONDULINE
compound belonging to the isothiazolinone class of broad- SA's instructions on overlapping.
spectrum microbiocides.
Octyl refers to the octyl group, which is a functional group
consisting of 8 carbon atoms. Isothiazolinone is a type of
heterocycle containing a five-membered ring composed of three
carbon atoms, one nitrogen atom and one sulphur atom.
Terbutryn is an aromatic heteromonocyclic compound
containing a methylthio-1,3,5-triazine and a diamino-1,3,5-
triazine.
2.9 Packaging
The final products are put onto wooden pallets and then
Zinc pyrithione is a coordination complex of zinc : zinc ; 1-
shrinkwrapped with polypropylene stretch foil and necessary
oxidopyridin-1-ium-2-thiolate.
registrations are done before the products are stored in the
warehouse.
No other ancillary materials or additives remain on the
products.
Possible reuse, recycling, energy recovery, and disposal routes
2.6 Manufacture of packaging materials :
Corrugated bitumen materials as sheets are made mainly from • For polypropylene stretch foil, it is considered that ratios
a single layer of natural cellulose fibres (secondary material) are: 28,2% landfill, 50,4% incineration with energy
that are recycled from all sources of wastepaper and recovery, 21,4% recycling and 0% re-use. A generic
cardboard, pre-pigmented with resin and colouring, and distance of 50km is considered between dismantling site
impregnated with bitumen, under pressure and heat. and waste treatment sites.
• For woodden pallets, it is considered that ratios are:
The production stage contains A1 (extraction, processing, 20% landfill, 31% incineration with energy recovery, 7%
production of raw materials), A2 (Transport to the manufacturer recycling and 42% re-use. It is also considered that the
and internal transport) and A3 (Manufacturing processes) transport distance from the dismantling site to the reuse
modules. site equals 200 km, whereas the transport distance to
Manufacturing steps of corrugated bitumen sheets are defined every other waste treatment sites (landfill, incineration
in detail as follows. The production process is the same for all and recycling) is considered to be 50km.
sites. The manufacturing process is composed of two main
sections: 2.10 Condition of use
There are no changes in material composition over the service
• Cardboard production section:
life of the product.
The incoming wastepaper is sorted, turned into pulp and
drained. All along, processes of degassing and impurity
2.11 Environment and health during use
separation are realised. Afterwards, the pulp made of
There are no environmental and health impacts related to the
fibres of cellulose and fillers is shaped and coloured. It
material composition during the use phase.
undergoes primary coating (application of colour, resin
and pigment based) and corrugation processes. 2.12 Reference service life
Cardboards are then heated and completely dried by
Service life has been declared by the manufacturer in line with
natural gas. The cardboards are cut into required
the BBSR table, the PCR (Part B, 2.12) and 15804+A2. It is
dimensions and passed onto the impregnation stage.
also based on the experience of under-roofing sheets
manufacture and supply. The service life is set at 50 years for
• Impregnation Section:
under-roofing applications.
In this section, cardboard gains its waterproofing
property. It is completely saturated with bitumen at high
A service life in accordance with the BBSR table is not a
temperatures. After impregnation, the sheets undergo
reference service life (RSL) according to ISO 15686.
curing and cooling operations.
For the packaging process, the finished products are put
The service life declared by the manufacturer only applies for
onto pallets and then shrink-wrapped with
the declared service life conditions.
Polypropylene stretch foil.
This means that the product will meet its functional
2.7 Environment and health during manufacturing
requirements for 50 years before replacement.
ONDULINE SA's plants are certified ISO 45001:2018
(Occupational health and safety management systems — 2.13 Extraordinary effects
Requirements with guidance for use) and ISO 14001 : 2004
Fire
(Environmental management systems — Requirements with
For all corrugated bitumen sheets by ONDULINE SA, the class
guidance for use).
of fire performance is E. According to the test method NBN
CEN/TS 1187 (test 2), external fire performance of the roofing
2.8 Product processing/Installation
systems (sheets + tiles) is Broof (t2).
During assembly, finished product packaging as well as
installation scraps are sent to waste treatment, electric
screwdrivers are used to install roofing sheets and their fixings.
This stage also induce overlapping losses. As a matter of fact,
when laying Onduline corrugated bitumen sheets, the
manufacturer requires the sheets to be overlapped to ensure
3 Environmental Product Declaration - ONDULINE SA - Corrugated bitumen sheets for under-roofing application
Fire protection
2.14 Re-use phase
Name Value Reuse, recycling and incineration with energy recovery are
Building material class E possible practices but have not been considered because they
Burning droplets d2 are not representative of the practices of ONDULINE SA's
customers.
Smoke gas development -
2.15 Disposal
Water ONDULINE SA confirmed that a 100% landfill scenario shall be
No extraordinary effect declared. considered. After an internal survey carried out by ONDULINE
SA, it has been shown that when dismantling their roofs, clients
Mechanical destruction would send their corrugated bitumen sheets directly to the
In the event of an accidental fire, fumes are released (soot, CO, waste collection site to be buried. Corrugated bitumen sheets
CO2, etc.). are classified: 17 03 02 (bituminous mixtures).
2.16 Further information
For further information, please contact ONDULINE SA through
its website at http://www. onduline.com
3. LCA: Calculation rules
The EPD covers individual products, which are grouped by type
3.1 Declared Unit of application and product families. To evaluate the impacts of
This EPD refers to a functional unit defined as follows: 1m² the group of products, each product has been evaluated
corrugated bitumen sheets for under-roofing application to individually. For all typologies, the created average product
ensure waterproofing and weather protection for a minimum according to the distribution of global sales is used as a
slope of 15% over 50 years. reference for the EPD.
The environmental profile is based on a weighted average, as This declaration is classified as an 'average product' as
the LCA results refer to the specified functional unit. calculated from overall production in several of the
Declared unit and mass reference manufacturer's plants according to PCR Part A : Calculation
Rules for the Life Cycle Assessment and Requirements on the
Name Value Unit
Project Report according to EN 15804+A2:2019 (version 1.3),
Grammage (weighted average value between
2.93 kg/m2 31 August 2021; www.bau-umwelt.de.
2020 and 2022)
Declared unit 1 m2 3.2 System boundary
The system boundary covers the entire life cycle of the product
Layer thickness (weighted average value
0.0025 m from the extraction of raw materials to the disposal of the
between 2020 and 2022)
product (cradle to grave). It also includes the module D.
This study aims to find the environmental impacts generated by 3.3 Estimates and assumptions
ONDULINE SA products throughout their life cycle. For this, the All raw materials used by ONDULINE SA have been
standards ISO 14040, ISO 14044, EN 15804 have been approximated by datasets found on Ecoinvent 3.8 database.
complied with regarding the quality of data for the following For a more detailed study, an on-site collection of data (i.e. a
criteria: collection of data on the production sites of ONDULINE SA's
• Time factor – LCI data are based on: suppliers) would be required to acquire detailed information on
- Where available, data collected specifically for this the products identified as having a high level of impact.
study at ONDULINE SA production sites in Spain,
Malaysia, Poland and Turkey. These data correspond to Waterproofing properties of ONDULINE SA's products depend
the average production based on the study of data from on bitumen type (road bitumen). The grades selected by
the years 2020-2021-2022. ONDULINE are such that the bitumen does not remain on the
- In the absence of specific data, generic data from the surface of the sheet, allowing the material to be waterproof and
Ecoinvent database 3.8 Allocation, cut-off by homogenous as required by EN 534 standard. We have
Classification (2022). This database is regularly updated assumed that the dataset found on Ecoinvent 3.8 database
and is representative of current processes. matched the bitumen formulation purchased by ONDULINE SA.
Instead of taking a global dataset, we narrowed the studied
• Geographical factor:
area to Europe (for factories in Poland and Spain), and to Rest
- Specific data come from the manufacturer's production
of the World (for factories in Malaysia and Turkey). This limits
sites in Spain, Malaysia, Poland and Turkey.
the possible difference between averaged bitumen formulation
- Generic data from the Ecoinvent database
per studied area and purchased bitumen formulations by each
representing European or Rest of the World processes
factory.
have been used for manufacturing stages where
available, otherwise global data are used.
Whenever possible country-specific data (e.g. electricity, ...)
was applied. When such data is missing, European, rest-of-the
• Technological factor – material shaping technology data
world or global datasets are preferred (e.g. resins, natural gas,
are based on:
etc.)
- Technologies used by the manufacturer for the
production processes of their products.
For transports: When multiple location applied to the same raw
- European or Global technologies depending on the
material or reference of product, weighted average of the
production site considered in the case of generic data.
distances were used. All raw materials, their amount, their
4 Environmental Product Declaration - ONDULINE SA - Corrugated bitumen sheets for under-roofing application
distance between suppliers/producers and ONDULINE SA's All input and output flows have been considered.
plants were collected from each plant. All sales figures were
also collected from each plant, as well as the related transport
• Module D
distances. All transports by lorry as well as transports by light
The Module D has been considered for this report. It does not
commercial vehicle have been modelled with a calculated
include the packaging (Polypropylene stretch foil and wood
Global dataset. Transports by container ship were modelled
pallet).
with Ecoinvent Global dataset.
3.5 Background data
All the bitumen waste from disposal phase have been modelled The data used to create the model within the LCA software
as going to sanitary landfill. Although some ONDULINE SA's Simapro 9.5 has been provided by ONDULINE SA. Generic
customers do not send their corrugated bitumen sheets to data has been taken from the Ecoinvent database 'Ecoinvent
landfill when they are dismantled, but rather to recycling or 3.8 – allocation cut-off by classification'.
reuse, we have conservatively assumed that all flows went to
landfill. ONDULINE SA did not have figures to give to EVEA. 3.6 Data quality
For this average EPD, geographical, technical, temporal as well
3.4 Cut-off criteria
as methodological representativity have been met:
The cut-off criteria used for this study follow the guidelines set
• Geographical coverage is global,
out in the PCR which conform to the EN15804, as follows:
• Production data are based on the years 2020 to 2022
- All inputs and outputs to a (unit) process are included in the
(this study is based on 3-year averaged data, as
calculation where the data is available.
provided by ONDULINE SA),
- A maximum of 1% of the total mass per unit process may be
• Technologies used by the manufacturer for the
omitted.
production processes have been used in the calculation,
- A maximum of 1% of the total renewable and non-renewable
and European or Global technologies depending on the
energy for a unit process may be omitted.
production site have been considered when generic
- A maximum of 5% of the total energy usage and mass per
data where to be used,
module may be omitted.
• Data quality assessment is compliant to EN15804+A2
This study does not include infrastructures, production tools,
standard.
factory construction, lighting, heating, cleaning, administration
All data was collected by ONDULINE SA in kg per kg of
department or employee transport, except in the case of data
product. The data was reported in kg per sqm in the Simapro
included in the generic databases.
tool.
• Modules A1-A5
A1 & A2: The raw and secondary materials as well as their Variability studies have shown that sales-weighted average
transport have been included in the calculation. products per country can have an impact of -12% to +74%
Packaging of waste paper (steel strapping around stacks of regarding average GWP (the highest rates are for Malaysia and
waste paper) as well as its transport have been included in the the lowest rates are for Spain). They have also shown that the
calculation. The other raw materials packaging and their references alone can have an impact of -27% to +83%
transport were negligible and have not been included in the regarding average GWP (highest rate is that of a Malaysian
calculation. reference and lowest rates is that of a Spanish reference).
A3: Energy consumption, production goods, production losses
and wastes, finished product packaging and the import of Malaysia has the highest overall carbon footprint. This is mainly
fixings have been included in the calculation. due to its electricity consumption (highest of the 5 countries
Internal transport via forklift within the factory (Forklifts studied), its energy mix, the averaged mass per square meter
employed are diesel, LPG or/and propane driven) has not been of finished product (2nd highest of the 5 countries) and the
included in the calculationdue to the lack of annual fuel transport distance of the finished product (2nd highest of the 5
consumption figures and because this consumption is countries).
negligible regarding the impact of raw materials.
A4: Transport of the finished products, their fixings and their 3.7 Period under review
packaging to the stockist and then the construction site have The period under review for the collection of production data
been included in the calculation. and the resulting averages runs from 2020 to 2022.
A5: Screwdriver electric consumption during installation,
installation scraps (cutting scraps), installation losses 3.8 Geographic Representativeness
(overlapping) and finished product packaging waste have been Land or region, in which the declared product system is
included in the calculation. manufactured, used or handled at the end of the product´s
lifespan: Global
• Module B1
There are no input or output flows associated with this module
for the products considered. 3.9 Allocation
VOC emissions have been neglected, moreover no data was
The manufacturing process does not generate any
available.
simultaneous co-products. No allocation has been made on the
• Module B2 production data.
According to the data provided by ONDULINE SA, the
consumption of water used when cleaning the roofs can be 3.10 Comparability
omitted. Basically, a comparison or an evaluation of EPD data is only
possible if all the data sets to be compared were created
• Modules B3-B7
according to EN 15804 and the building context, respectively
There are no input or output flows associated with these
the product-specific characteristics of performance, are taken
modules for the products considered.
into account. Ecoinvent database 'Ecoinvent 3.8 – allocation
• Modules C1-C4 cut-off by classification' has been used.
5 Environmental Product Declaration - ONDULINE SA - Corrugated bitumen sheets for under-roofing application
4. LCA: Scenarios and additional technical information
The waste treatment of finished product packaging
Characteristic product properties of biogenic carbon (polypropylene stretch foil and wood pallets) has been
In this LCA, biogenic carbon content has been quantified and modelled with generic data created by EVEA. For wooden
declared for wooden pallets (packaging) and cardboard pallets, it is considered that ratios are: 20% landfill, 31%
contained in the corrugated bitumen sheets. incineration with energy recovery, 7% recycling and 42% re-
use. For polypropylene stretch foil, it is considered that ratios
Note: 1 kg of biogenic carbon is equivalent to 44/12 kg of CO 2. are: 28,2% landfill, 50,4% incineration with energy recovery,
21,4% recycling and 0% re-use. A generic distance of 50km is
Information on describing the biogenic carbon content at
considered between dismantling site and waste treatment sites.
factory gate
Name ValueUnit
Use or application of the installed product (B1)
kg There are no input or output flows associated with this module
Biogenic carbon content in product (Cardboard) 0.45
C for the products considered.
Biogenic carbon content in accompanying kg
0.47
packaging (Wooden pallet) C ONDULINE SA's corrugated bitumen sheets for under-roofing
applications have 50 years of service lifetime.
Note: 1 kg of biogenic carbon is equivalent to 44/12 kg of CO .
2
Service life
The service life declared by the manufacturer (50 years) only
The following is the technical scenario information used for applies for the declared service life conditions.
declared modules. Name Value Unit
Transport to the building site (A4) Life Span (according to BBSR) 50 years
The transport of the final products has been modelled by Application under-roofing
considering their precise destinations in the world. For each Declared product properties (at EN 534:2006+A1 EN
-
product family, a transport distance averaged by sales volumes the gate) and finishes 14964:2006
for each destination has been taken. The transported mass of
Design application parameters See ONDULINE SA
packaging of the finished products as well as the transported
(if instructed by the technical book and
mass of fixings needed for the installation stage are included in
manufacturer), including the instructions on reference -
the calculation at this stage. Lorry and container ship generic
references to the appropriate conditions of application
models used are globally representative. A third transport
practices and application codes and use
model has been created here to consider a generic distance of
See ONDULINE SA
a 100km covered by a light commercial vehicle between the An assumed quality of work,
technical book and
stockist and the building site. This model is also globally when installed in accordance
instructions on reference -
representative. with the manufacturer’s
conditions of application
Name Value Unit instructions and use
Transport distance by truck 1025 km Outdoor environment, (for
Transport distance by container ship 724 km outdoor applications), e.g.
Transport distance by light commercial vehicule 100 km weathering, pollutants, UV and
No specific restrictions -
wind exposure, building
Installation into the building (A5) orientation, shading,
Distribution packaging consists of wooden pallets (2,77E-02 temperature
kg/m²) and polypropylene stretch foil (1,46E-03 kg/m²). Usage conditions, e.g.
Electric screwdrivers are used to fix sheets to the roofing. frequency of use, mechanical No specific restrictions -
ONDULINE SA has estimated the screwdriver's electric exposure
consumption at 0,0025 kWh per kg of installed product
Maintenance e.g. required
regardless of the reference. The electric consumption is
frequency, type and quality and No specific restrictions -
converted in kWh per m² of product before being integrated in
replacement of components
SimaPro. As ONDULINE SA products are sold all over the
world, the Ecoinvent data is representative of the world. End of life (C1-C4)
Name Value Unit The same energy consumption as in A5 has been considered,
Electricity consumption 0.008 kWh given that electric screwdrivers are also used to remove sheets
from the roof.Corrugated bitumen sheets and fixings are sent
Installation scraps 3 %
by truck to their waste treatment and their recycling sites 50 km
Overlapping losses depend on the reference of sheets, they are away.
around 17-20%. They have been modelled with only a demand 100 % of the fixings are recycled.
of overproduction to offset the losses. No waste treatment has 100 % of the corrugated bitumen sheets are landfilled.
been modelled. The scraps associated with the installation,
Name ValueUnit
entirely in the form of offcuts, are estimated at 3% by
Collected separately waste type (Fixings) 0.039 kg
ONDULINE SA. They have been modelled with overproduction
to offset the scraps and with a waste treatment. According to Collected separately (Corrugated bitumen sheets) 3.338 kg
ONDULINE SA's information, end-of-life scenario to be Recycling (Fixings) 0.039 kg
considered for installation scraps is 100% landfill. All these Landfilling (Corrugated bitumen sheets) 3.338 kg
scraps are transported by truck to the landfill site, assumed to
Recycling potentials (D), relevant scenario information
be 50km away. It is modelled with a
The recycling of fixings is considered in module D.
global lorry data.
Module D includes the credits of the recycling of fixings (100%)
6 Environmental Product Declaration - ONDULINE SA - Corrugated bitumen sheets for under-roofing application
from C3, considering that 26% of the fixings contain recycled steel.
7 Environmental Product Declaration - ONDULINE SA - Corrugated bitumen sheets for under-roofing application
5. LCA: Results
DESCRIPTION OF THE SYSTEM BOUNDARY (X = INCLUDED IN LCA; MND = MODULE OR INDICATOR NOT DECLARED; MNR
= MODULE NOT RELEVANT)
Benefits and
Construction loads beyond
Product stage Use stage End of life stage
process stage the system
boundaries
la ire ta m w a Ry lp p u s tro p s n a rT g n iru tc a fu n a M e h t m o rf tro p s n a rTe tis e h t o t e ta g y lb m e s s A e s U e c n a n e tn ia M ria p e R tn e m e c a lp e R tn e m h s ib ru fe R y g re n e la n o ita re p Oe s u re ta w la n o ita re p Oe s u n o itc u rts n o c -e Dn o itilo m e d tro p s n a rT g n is s e c o rp e ts a W la s o p s iD -e s u e R-y re v o c e R-g n ilc y c e Rla itn e to p
A1 A2 A3 A4 A5 B1 B2 B3 B4 B5 B6 B7 C1 C2 C3 C4 D
X X X X X X X X X X X X X X X X X
RESULTS OF THE LCA - ENVIRONMENTAL IMPACT according to EN 15804+A2: 1 m² of under-roof waterproofed and
protected by corrugated bitumen sheets for a minimum slope of 15% and a lifespan of 50 years
Parameter Unit A1 A2 A3 A4 A5 B1 B2 B3 B4 B5 B6 B7 C1 C2 C3 C4 D
GWP-total kg CO 2 -1.64E 9.64E- 1.25E 1.13E 4E-01 0 0 0 0 0 0 0 4.21E- 2.87E- 3.03E- 3.21E -2.57E-
eq +00 02 +00 +00 03 02 03 +00 02
GWP-fossil kg CO 2 8E-01 9.63E- 1.14E 1.13E 5.79E-01 0 0 0 0 0 0 0 4.19E- 2.87E- 3.02E- 4.26E- -2.58E-
eq 02 +00 +00 03 02 03 01 02
GWP- kg CO 2 -2.44E 2.86E- 1.11E- 5.92E- -1.81E- 0 0 0 0 0 0 0 1.14E- 8.52E- 4.68E- 2.78E 3.45E-05
biogenic eq +00 05 01 04 01 05 06 06 +00
GWP-luluc kg CO 2 6.16E- 4.04E- 1.71E- 6.38E- 1.49E-03 0 0 0 0 0 0 0 1E-05 1.2E-05 2.36E- 4.1E-05 1.85E-05
eq 03 05 03 04 06
kg CFC11 2.17E- 1.09E- 2.42E- 1.45E- 6.47E- 5.47E- 1.07E- -7.72E-
ODP 1.1E-06 2.51E-07 0 0 0 0 0 0 0
eq 08 07 07 10 09 10 08 10
8.85E- 4.12E- 3.62E- 6.16E- 2.17E- 1.19E- 1.42E- -1.11E-
AP mol H+ eq 3.37E-03 0 0 0 0 0 0 0 5.4E-04
03 04 03 03 05 04 05 04
EP- 1.24E- 7.79E- 3.34E- 1.26E- 2.24E- 2.32E- 5.26E- 6.42E- -9.62E-
kg P eq 1.16E-05 0 0 0 0 0 0 0
freshwater 05 07 05 05 07 07 08 07 08
1.08E- 1.79E- 3.64E- 3.49E- 3.53E- 4.29E- -4.08E-
EP-marine kg N eq 1.1E-03 1.2E-04 7.38E-04 0 0 0 0 0 0 0
03 03 06 05 06 04 06
1.27E- 1.33E- 7.55E- 1.98E- 4.08E- 3.86E- 4.31E- 1.15E- -2.88E-
EP-terrestrial mol N eq 7.36E-03 0 0 0 0 0 0 0
02 03 03 02 05 04 05 03 04
kg
4.81E- 4.03E- 2.64E- 6.18E- 1.18E- 1.17E- 4.54E- -1.55E-
POCP NMVOC 2.48E-03 0 0 0 0 0 0 0 1.1E-05
03 04 03 03 04 05 04 04
eq
3.41E- 2.81E- 1.06E- 1.02E- 1.27E- -8.23E-
ADPE kg Sb eq 4.3E-06 3.23E-06 0 0 0 0 0 0 0 2E-08 1.3E-08
07 06 05 07 07 07
6.86E 1.44E 1.86E 1.68E 1.81E 5.58E- 4.35E- -2.18E-
ADPF MJ 0 0 0 0 0 0 0 4.3E-01 8.5E-01
+01 +00 +01 +01 +01 02 02 01
m3 world
2.78E- 4.79E- 2.75E- 6.98E- 1.43E- 2.44E- 3.63E-
WDP eq 7.1E-02 1.19E-01 0 0 0 0 0 0 0 7.02E-03
01 03 01 04 03 04 02
deprived
GWP = Global warming potential; ODP = Depletion potential of the stratospheric ozone layer; AP = Acidification potential of land and water; EP =
Eutrophication potential; POCP = Formation potential of tropospheric ozone photochemical oxidants; ADPE = Abiotic depletion potential for non-fossil
resources; ADPF = Abiotic depletion potential for fossil resources; WDP = Water (user) deprivation potential)
RESULTS OF THE LCA - INDICATORS TO DESCRIBE RESOURCE USE according to EN 15804+A2: 1 m² of under-roof
waterproofed and protected by corrugated bitumen sheets for a minimum slope of 15% and a lifespan of 50 years
Parameter Unit A1 A2 A3 A4 A5 B1 B2 B3 B4 B5 B6 B7 C1 C2 C3 C4 D
4.59E- 1.77E- 3.14E- 7.24E- 5.27E- 1.84E- 1.69E- -3.03E-
PERE MJ 1.5E+00 9.8E-01 0 0 0 0 0 0 0
01 02 01 03 03 03 02 02
2.81E 1.38E 3.76E
PERM MJ 0 0 0 0 0 0 0 0 0 0 0 0 0 0
+01 +00 +00
2.85E 1.77E- 2.88E 3.14E- 4.74E 7.24E- 5.27E- 1.84E- 1.69E- -3.03E-
PERT MJ 0 0 0 0 0 0 0
+01 02 +00 01 +00 03 03 03 02 02
1.01E 1.44E 1.81E 1.67E 8.32E 5.56E- 4.35E- -2.18E-
PENRE MJ 0 0 0 0 0 0 0 4.3E-01 8.5E-01
+01 +00 +01 +01 +00 02 02 01
6.31E 4.85E- 1.06E
PENRM MJ 0 0 0 0 0 0 0 0 0 0 0 0 0 0
+01 01 +01
7.32E 1.44E 1.86E 1.67E 1.89E 5.56E- 4.35E- -2.18E-
PENRT MJ 0 0 0 0 0 0 0 4.3E-01 8.5E-01
+01 +00 +01 +01 +01 02 02 01
1.48E 1.54E- 2.52E-
SM kg 0 0 0 0 0 0 0 0 0 0 0 0 0 0
+00 02 01
RSF MJ 0 0 0 0 0 0 0 0 0 0 0 0 0 0 0 0 0
NRSF MJ 0 0 0 0 0 0 0 0 0 0 0 0 0 0 0 0 0
1.04E- 2.33E- 3.82E- 3.28E- 4.49E- 8.91E- 8.77E-
FW m3 7.2E-03 1.5E-04 0 0 0 0 0 0 0 2.91E-04
02 03 03 05 05 06 04
8 Environmental Product Declaration - ONDULINE SA - Corrugated bitumen sheets for under-roofing application
PERE = Use of renewable primary energy excluding renewable primary energy resources used as raw materials; PERM = Use of renewable primary
energy resources used as raw materials; PERT = Total use of renewable primary energy resources; PENRE = Use of non-renewable primary energy
excluding non-renewable primary energy resources used as raw materials; PENRM = Use of non-renewable primary energy resources used as raw
materials; PENRT = Total use of non-renewable primary energy resources; SM = Use of secondary material; RSF = Use of renewable secondary fuels;
NRSF = Use of non-renewable secondary fuels; FW = Use of net fresh water
RESULTS OF THE LCA – WASTE CATEGORIES AND OUTPUT FLOWS according to EN 15804+A2:
1 m² of under-roof waterproofed and protected by corrugated bitumen sheets for a minimum slope of 15% and a lifespan of 50
years
Parameter Unit A1 A2 A3 A4 A5 B1 B2 B3 B4 B5 B6 B7 C1 C2 C3 C4 D
2.68E- 1.32E- 4.93E- 2.27E- 2.64E- 1.89E- 3.93E- 6.08E- 1.21E- -1.36E-
HWD kg 0 0 0 0 0 0 0
02 03 02 02 02 04 04 04 03 02
2.66E- 8.34E- 7.44E- 9.02E- 4.65E- 2.92E- 2.49E- 2.67E- 3.35E -3.72E-
NHWD kg 0 0 0 0 0 0 0
01 02 01 01 01 03 02 03 +00 02
4.68E- 9.48E- 3.99E- 1.09E- 1.07E- 1.72E- 2.82E- 2.53E- 4.98E-
RWD kg 0 0 0 0 0 0 0 1.62E-07
04 06 05 04 04 07 06 07 06
3.99E-
CRU kg 0 0 0 0 0 0 0 0 0 0 0 0 0 0 0 0
02
7.71E- 3.86E-
MFR kg 0 0 0 0 0 0 0 0 0 0 0 0 0 0 0
03 02
MER kg 0 0 0 0 0 0 0 0 0 0 0 0 0 0 0 0 0
4.77E-
EEE MJ 0 0 0 0 0 0 0 0 0 0 0 0 0 0 0 0
02
9.96E-
EET MJ 0 0 0 0 0 0 0 0 0 0 0 0 0 0 0 0
02
HWD = Hazardous waste disposed; NHWD = Non-hazardous waste disposed; RWD = Radioactive waste disposed; CRU = Components for re-use;
MFR = Materials for recycling; MER = Materials for energy recovery; EEE = Exported electrical energy; EET = Exported thermal energy
RESULTS OF THE LCA – additional impact categories according to EN 15804+A2-optional:
1 m² of under-roof waterproofed and protected by corrugated bitumen sheets for a minimum slope of 15% and a lifespan of 50
years
Parameter Unit A1 A2 A3 A4 A5 B1 B2 B3 B4 B5 B6 B7 C1 C2 C3 C4 D
Disease 5.44E- 8.26E- 2.44E- 1.09E- 3.57E- 1.62E- 2.47E- 2.46E- 6.23E- -1.42E-
PM 0 0 0 0 0 0 0
incidence 08 09 08 07 08 10 09 10 09 09
kBq U235 2.86E- 6.02E- 5.08E- 7.09E- 7.16E- 2.49E- 1.79E-
IR 0 0 0 0 0 0 0 1.8E-04 3.3E-03 3.86E-04
eq 01 03 02 02 02 04 03
2.01E 5.16E- 3.72E 5.94E 5.33E 1.38E- 1.54E- 1.57E- 7.41E-
ETP-fw CTUe 0 0 0 0 0 0 0 4.75E-02
+01 01 +00 +00 +00 02 01 02 01
1.97E- 3.68E- 1.16E- 1.35E- 1.24E- 1.09E- 1.43E- 2.81E-
HTP-c CTUh 1.1E-09 0 0 0 0 0 0 0 2.57E-10
09 11 09 09 12 11 12 11
1.08E- 9.11E- 1.79E- 7.89E- 4.47E- 3.57E- 3.71E- 4.37E-
HTP-nc CTUh 1.2E-09 0 0 0 0 0 0 0 1.55E-09
08 09 08 09 11 10 11 10
8.67E 1.64E 9.47E 6.81E 9.02E- 2.93E- 3.24E- 1.98E -1.06E-
SQP SQP 9.8E-01 0 0 0 0 0 0 0
+00 +01 +00 +00 03 01 02 +00 01
PM = Potential incidence of disease due to PM emissions; IR = Potential Human exposure efficiency relative to U235; ETP-fw = Potential comparative
Toxic Unit for ecosystems; HTP-c = Potential comparative Toxic Unit for humans (cancerogenic); HTP-nc = Potential comparative Toxic Unit for humans
(not cancerogenic); SQP = Potential soil quality index
Disclaimer 1 – for the indicator 'Potential Human exposure efficiency relative to U235'. This impact category deals mainly with the
eventual impact of low-dose ionizing radiation on human health of the nuclear fuel cycle. It does not consider effects due to possible
nuclear accidents, occupational exposure or radioactive waste disposal in underground facilities. Potential ionizing radiation from the
soil, radon and from some construction materials is also not measured by this indicator.
Disclaimer 2 – for the indicators 'abiotic depletion potential for non-fossil resources', 'abiotic depletion potential for fossil resources',
'water (user) deprivation potential, deprivation-weighted water consumption', 'potential comparative toxic unit for ecosystems', 'potential
comparative toxic unit for humans – cancerogenic', 'Potential comparative toxic unit for humans - not cancerogenic', 'potential soil
quality index'. The results of this environmental impact indicator shall be used with care as the uncertainties on these results are high
as there is limited experience with the indicator.
As no RSL is declared according to ISO 15686, the LCA results of the modules B1-B2 and B6-B7 refer to a period of one year.
This EPD was created using a software tool.
6. LCA: Interpretation
For all products, the stages with the greatest environmental Photochemical ozone formation, Resource use (minerals,
impacts are: the raw materials supply stage (A1), the metals and fossils), Water use, Particulate matter, Ionising
manufacturing stage (A3), the delivery transport stage (A4), the radiation, Human toxicity (cancer and non-cancer), Total non-
installation stage (A5), the end of life – disposal phase (C4). renewable primary energy, Net use of fresh water, Hazardous
waste disposed, Radioactive waste disposed, Interm. & low-
The raw material supply is responsible for over 20% of the level radioactive waste, Exported energy and Total primary
impact for following indicators: Climate change – fossil, Climate energy. It is mostly always due to the supply of bitumen, for
change - land use and change, Ozone depletion, Acidification, some indicators, it is also due to the supply of resin and for a
Eutrophication (freshwater, marine and terrestrial), few indicators it is partly due to the supply of pigments.
9 Environmental Product Declaration - ONDULINE SA - Corrugated bitumen sheets for under-roofing application
Distribution of impacts for the sales weighted average product
The raw material supply is also responsible for over 70% of the (under-roofing application, LCA results over the full service life)
impact for following indicators: Renewable primary energy used
as RM, Total renewable primary energy, Non-renewable Variability studies have shown that sales-weighted average
primary energy used as RM and Use of secondary material. It is products per country can have an impact of -12% to +74%
always due to the supply of cardboard, except for the indicator regarding average GWP (the highest rates are for Malaysia and
'Non-renewable primary energy used as RM', for which it is due the lowest rates are for Spain). They have also shown that the
to the supply of bitumen. references alone can have an impact of -27% to +83%
regarding average GWP (highest rate is that of a Malaysian
The manufacturing stage is responsible for over 30% of the reference and lowest rates is that of a Spanish reference).
impact for following indicators:
Considering the high results variability, the environmental
• Climate change - land use and change, Eutrophication
profile of a sub-group of products or individual products are
(freshwater), Net use of fresh water and High-level
available upon request.
radioactive waste, due to the electric consumption,
• Land use and Renewable primary energy excl. RM, due
to the supply of wood pallets,
• Climate change – fossil and Non-renewable primary
energy excl. RM, due to the consumption of natural gas,
• Hazardous waste disposed, due to the supply of fixings.
The transport stage (finished product transport – A4) is
responsible for over 25% of the impact for following indicators:
Eutrophication (marine and terrestrial), Photochemical ozone
formation, Resource use (minerals and metals), Particulate
matter, Human toxicity (non-cancer), Non-renewable primary
energy excl. RM, always and overwhelmingly due to the
delivery by light commercial vehicle from stockist to worksite.
The installation stage (A5) is responsible for over 15% of the
impact for all the indicators studied in EN15804 standard
(except Climate change – biogenic and total, Use of renewable
secondary fuels, Use of non-renewable secondary fuels, Non-
hazardous waste disposed, Materials for recycling, Materials for
energy recovery, Exported energy - gas and process), mainly
due to the overproduction needed to offset the overlapping
rates and for a few indicators, it is also due also to the end of
life of the wooden pallets.
Finally, the disposal stage (C4) is responsible for over 40% of
the impact for following indicators: Climate change – total,
Climate change – biogenic, Non-hazardous waste disposed,
due to the landfilling of waste bitumen sheets.
10 Environmental Product Declaration - ONDULINE SA - Corrugated bitumen sheets for under-roofing application
7. Requisite evidence
External fire performance and reaction to fire of the roofing
systems (sheets + tiles). Wind Driven Rain Testing of Onduline Roofing Underlay System
to EN 15601.
Test standard: CEN/TS 1187-T1 (test 2)
Classification standard: EN 13501-1:2016 and EN 13501- Test standard: type B and type D test from prEN 15601
5:2016 Classification standard: EN 15601
Measuring agency: Warrington fire, WFRGENT nv Measuring agency: BRE, Building Research Establishment Ltd
Results of the measurement: Class of external fire performance Results of the measurement: Onduline Roofing Underlay
is Broof for every product. Class of fire reaction is E for every System exceed the minimum Pressure Factor target of 30Pa
product. set by BBA for a 10° roof pitch.
8. References
EN 534:2006+A1:2010 procedures.
Corrugated bitumen sheets-Product specification and test
method ISO 14040-44
DIN EN ISO 14040:2006: Environmental management - Life
EN 13501-1:2016 cycle assessment - Principles and framework (ISO 14040:2006)
BS EN 13501-1:2016, Fire classification of construction and Requirements and guidelines (ISO 14044:2006)
products and building elements - Part1: Classification using
data from reaction to fire tests Regulation (EU) No. 305/2011 (CPR)
Harmonised conditions for the marketing of construction
EN 13501-5 products
NBN EN 13501-5, Fire classification of construction products
and building elements - Part 5: Classification using data from Database Ecoinvent
external fire exposure to roofs tests Ecoinvent v3.8 (2022 - Ecoinvent Centre)
According to test method NBN CEN/TS 1187 (test 2), external
performance of the roofing systems (sheets + tiles) is Broof (t2). IBU 2021
Institut Bauen und Umwelt e.V.: General Instructions for the
EN 14964:2006 EPD programme of Institut Bauen und Umwelt e.V., Version
Rigid underlays for discontinuous roofing – type OL - Definitions 2.0, Berlin: Institut Bauen und Umwelt e.V., 2021
and characteristics www.ibu-epd.com
EN 15804 PCR Part A
EN 15804:2012+A2:2019+AC:2021, Sustainability of Institut Bauen und Umwelt e.V., Berlin (pub.): Product Category
construction works — Environmental Product Declarations — Rules for Construction Products from the range of
Core rules for the product category of construction products. Environmental Product Declarations of Institut Bauen und
Umwelt (IBU). Part A: Calculation Rules for the Life Cycle As-
ISO 9001 : 2008 sessment and Requirements on the Project Report according to
Quality management systems — Requirements EN 15804+A2:2019 (version 1.3), 31 August 2021; www.bau-
umwelt.de
ISO 14001 : 2004
Environmental management systems — Requirements with PCR Part B
guidance for use. Institut Bauen und Umwelt e.V., Berlin (pub.): Product Category
Rules for Construction Products from the range of
ISO 45001:2018 Environmental Product Declarations of Institut Bauen und
Occupational health and safety management systems — Umwelt (IBU), Part B: Requirements on the EPD for corrugated
Requirements with guidance for use. bitumen materials for roofing and external wall cladding, 1 June
2021, www.bau-umwelt.de
ISO 14025
EN ISO 14025:2011, Environmental labels and declarations — Software Simapro
Type III environmental declarations — Principles and SimaPro 9.5 (2023 - Pré consultant)
11 Environmental Product Declaration - ONDULINE SA - Corrugated bitumen sheets for under-roofing application
Publisher
Institut Bauen und Umwelt e.V. +49 (0)30 3087748- 0
Hegelplatz 1 info@ibu-epd.com
10117 Berlin www.ibu-epd.com
Germany
Programme holder
Institut Bauen und Umwelt e.V. +49 (0)30 3087748- 0
Hegelplatz 1 info@ibu-epd.com
10117 Berlin www.ibu-epd.com
Germany
Author of the Life Cycle Assessment
EVEA +33 2 28 07 87 00
rue Arthur III, 11 contact@evea-conseil.com
44200 Nantes www.evea-conseil.com/en
France
Owner of the Declaration
ONDULINE SA +33 1 55 63 80 10
Quai Gallieni 24 info@onduline.fr
92150 SURESNES www.onduline.com
France
12 Environmental Product Declaration - ONDULINE SA - Corrugated bitumen sheets for under-roofing application
