ENVIRONMENTAL PRODUCT DECLARATION
as per ISO 14025 and EN 15804+A2
Owner of the Declaration VELUX Group
Publisher Institut Bauen und Umwelt e.V. (IBU)
Programme holder Institut Bauen und Umwelt e.V. (IBU)
Declaration number EPD-VEL-20220032-CBE4-EN
Issue date 24.05.2022
Valid to 23.05.2027
VELUX PUR roof windows (62 triple glazing configuration)
VELUX Group
www.ibu-epd.com | https://epd-online.com
General Information
VELUX Group VELUX PUR roof windows (62 triple glazing
configuration)
Programme holder Owner of the declaration
IBU – Institut Bauen und Umwelt e.V. VELUX Group
Hegelplatz 1 Ådalsvej 99
10117 Berlin 2970 Hørsholm
Germany Denmark
Declaration number Declared product / declared unit
EPD-VEL-20220032-CBE4-EN The declared unit is a PUR roof window of one square meter (m2) with the
triple glazing configuration 62.
The declared unit is based on the configuration of a standard size window
measuring 1.23 m * 1.48 m.
This declaration is based on the product category rules: Scope:
Windows and doors , 01.08.2021 The EPD is a representative EPD covering VELUX PUR roof windows as
(PCR checked and approved by the SVR) specified in more detail in the product description. The products are
manufactured by the VELUX Group at production sites in different
locations in Europe for sale throughout Europe.
Issue date The owner of the declaration shall be liable for the underlying information
and evidence; the IBU shall not be liable with respect to manufacturer
24.05.2022
information, life cycle assessment data and evidences.
The EPD was created according to the specifications of EN 15804+A2. In
Valid to
the following, the standard will be simplified as EN 15804.
23.05.2027
Verification
The standard EN 15804 serves as the core PCR
Independent verification of the declaration and data according to ISO
14025:2011
internally X externally
Dipl.-Ing. Hans Peters
(Chairman of Institut Bauen und Umwelt e.V.)
Florian Pronold Juliane Franze,
(Managing Director Institut Bauen und Umwelt e.V.) (Independent verifier)
1 Environmental Product Declaration - VELUX Group - VELUX PUR roof windows (62 triple glazing configuration)
Product
was assessed to be a conservative choice for a representative
Product description/Product definition window type.
The VELUX polyurethane (PUR) roof windows are skylight
window products for sale in the European market. The product The glass panes are with triple glazing configuration 62 with a
family covers a range of product varieties as specified in the glass thickness of 17 mm. The glass panes have cavities filled
table on page 3. All the windows have a PUR frame/sash with a with Krypton gas.
wooden core. Some windows can be opened (venting), while
others cannot be opened (fixed). Some of the window varieties Only the window modules are included, which means that any
can be used in conjunction with electronic devices for automatic applied electronics, additional equipment, engines etc. are not
opening and closing, while other windows are opened and part of the EPD.
closed manually. The calculations are based on the
representative window type named GPU. In the LCA, the GPU
For the placing on the market of the product in the European specific values can be selected at the bottom of the above-
Union/European Free Trade Association (EU/EFTA) (with the mentioned download page.
exception of Switzerland) Regulation (EU) No. 305/2011 (CPR)
Constructional data (Reference product GPU incl. pane
applies. The product needs a declaration of performance taking
variant 62. For other variation, see velux.com/ce)
into consideration EN 14351-1:2006+A2:2016, Windows and
doors - Product standard, performance characteristics - Part 1:
Windows and external pedestrian doorsets. For the application
and use, the respective national provisions apply.
Application
VELUX PUR roof windows are used in renovation and new
build. Either installed as a single window or in a combination of
multiple windows.
Technical Data
The Declaration of Performance including relevant technical
specifications and test methods/test standards can be
downloaded from the website www.velux.com/ce.
The performance values are specific for each PUR roof window
variant covered by the EPD.
The declared values in the table relate to the reference product
incl. an average pane. For other covered product variants,
2 Environmental Product Declaration - VELUX Group - VELUX PUR roof windows (62 triple glazing configuration)
Name Value Unit 1:2006+A2:2016, Windows and doors - Product standard,
performance characteristics - Part 1: Windows and external
Fire resistance class § 4.4.1 D-s2.d2 class
pedestrian doorsets.
Air permeability , § 4.14 4 class
Resistance to wind load, § Base materials/Ancillary materials
4.2 (for window width >1140 C3 class Name Value Unit
mm or height > 1398 mm no
Glazing unit 57 %
performance is determined)
PUR/wooden frame 20 %
8 mm toughened - 11
Galvanized steel components 15 %
Resistance to snow loads, § mm - 3 mm heat
mm
4.3 strengthened - 11 mm - Other materials 8 %
6.8 mm laminated float
This product/article/at least one partial article contains
Watertightness, § 4.5 E900 class substances listed in the candidate list (date:
Impact resistance, § 4.7 (for 07.03.2022) exceeding 0.1 percentage by mass: NO.
window width <550 mm or
3 class
height <778 mm no Recycled content
performance is determined)
Load-bearing capacity of
test is passed -
safety devices, § 4.8
Acoustic performance, §
42 (-2; -5) -
4.11
The values stated in the table relate to the recycled material
Thermal transmittance, §
streams in VELUX production.
4.12 , 90 degree installation 0,96 W/(m2K)
acc. to EN 10077-1/2
Solar factor, § 4.13 0.47 - Reference service life
Light transmittance, § 4.13 0.68 - No reference service life (RSL) is defined for the roof windows
because the use stage modules are not included in the EPD.
Product performance data in accordance with DS/EN 14351-
LCA: Calculation rules
windows take place, which involves shortening of
Declared Unit profiles, drilling of holes, clamping and glueing,
Multiple product dimensions are represented by this EPD as mounting of gaskets, brackets, panes etc. as well as
specified in the product description. stacking on pallets.
The declared unit is 1 m2 window calculated based on one
representative window module measuring 1.23 m * 1.48 m End of life stage:
(reference window based on EN 14351-1) with triple glazed
• C1 - De-construction/demolition: de-construction of the
window panes.
window with the use of an electric screwdriver
Declared unit
• C2 - Transport: transport of window materials to
Name Value Unit incineration and recycling
conversion factor 57.7 -
• C3 - Waste processing: sorting of glass waste,
Declared unit 1 m2 incineration of plastic and rubber parts
A data quality and a sensitivity analysis show that the results • C4 - Disposal: disposal of all materials
are robust with regard to data quality and appropriateness. Benefits and loads beyond the system boundaries:
There is low variability of production processes and product • D - Reuse, recovery and recycling potential: benefits
variations have a limited influence on the results. from plastic incineration processes and material
recycling of metal and glass.
System boundary
Type of EPD: Cradle to gate - with options. The following life Geographic Representativeness
cycle phases were considered: Land or region, in which the declared product system is
Product stage: manufactured, used or handled at the end of the product´s
• A1 - Raw material supply: extraction and processing, lifespan: Europe
production of the pre-products (e.g. laminated glass,
brackets, sealant...) and packaging components
Comparability
(primarily cardboard)
Basically, a comparison or an evaluation of EPD data is only
• A2 - Transport: Transport of pre-products and packaging
possible if all the data sets to be compared were created
components to the manufacturing sites
according to EN 15804 and the building context, respectively
• A3 - Manufacturing: The PUR profiles and the panes are the product-specific characteristics of performance, are taken
produced internally at VELUX production sites. into account.
Subsequently, the final production and assembly of the
LCA: Scenarios and additional technical information
Characteristic product properties of biogenic carbon
3 Environmental Product Declaration - VELUX Group - VELUX PUR roof windows (62 triple glazing configuration)
6.9 kg of wood is used in the core window frames and 3.1 kg of
cardboard packaging is used per declared unit.
End of life (C1-C4)
Information describing the biogenic Carbon Content at Name Value Unit
factory gate
Collected as mixed construction waste 58 kg
Name ValueUnit
Recycling 21 kg
kg
Biogenic carbon content in product 3.6 Energy recovery 13 kg
C
Landfilling 24 kg
Biogenic carbon content in accompanying kg
2.5
packaging C Reuse, recovery and/or recycling potentials (D), relevant
Note: 1 kg of biogenic carbon is equivalent to 44/12 kg of CO . scenario information
2
The recycling efficiency for all materials is maximum 90 % in
accordance with EN 17213. This means that only 90 % of the
The construction process stage and the use stage modules are recycled materials substitute primary materials. Secondary
not declared. However, the quantity of packaging generated in materials in the windows do not substitute primary materials in
module A5 is declared as scenario information. the end-of-life scenario. The recycled glass is used as container
glass in the end-of-life scenario.
Installation into the building (A5)
Name Value Unit
Name ValueUnit
Glass recycled 30 %
Cardboard packaging for waste treatment 3.1 kg
Metal recycled 95 %
Plastic packaging (primarily EPS) for waste
0.3 kg Plastic incinerated with energy recovery 95 %
treatment
4 Environmental Product Declaration - VELUX Group - VELUX PUR roof windows (62 triple glazing configuration)
LCA: Results
DESCRIPTION OF THE SYSTEM BOUNDARY (X = INCLUDED IN LCA; MND = MODULE OR INDICATOR NOT DECLARED; MNR
= MODULE NOT RELEVANT)
Benefits and
Construction loads beyond
Product stage Use stage End of life stage
process stage the system
boundaries
la ire ta m w a Ry lp p u s tro p s n a rT g n iru tc a fu n a M e h t m o rf tro p s n a rTe tis e h t o t e ta g y lb m e s s A e s U e c n a n e tn ia M ria p e R tn e m e c a lp e R tn e m h s ib ru fe R y g re n e la n o ita re p Oe s u re ta w la n o ita re p Oe s u n o itc u rts n o c -e Dn o itilo m e d tro p s n a rT g n is s e c o rp e ts a W la s o p s iD -e s u e R-y re v o c e R-g n ilc y c e Rla itn e to p
A1 A2 A3 A4 A5 B1 B2 B3 B4 B5 B6 B7 C1 C2 C3 C4 D
X X X MND MND MND MND MNR MNR MNR MND MND X X X X X
RESULTS OF THE LCA - ENVIRONMENTAL IMPACT according to EN 15804+A2: 1 m2 Roof windows with triple glazing
Parameter Unit A1 A2 A3 C1 C2 C3 C4 D
GWP-total kg CO 2 eq 1.7E+02 3.84E+00 1.57E+01 1.84E-03 1.63E-01 2.73E+01 1.23E+00 -4.04E+01
GWP-fossil kg CO 2 eq 1.88E+02 3.82E+00 1.31E+01 1.82E-03 1.62E-01 1.5E+01 4.8E-01 -4.03E+01
GWP-biogenic kg CO 2 eq -1.81E+01 -4.86E-03 2.52E+00 1.55E-05 -2.06E-04 1.24E+01 7.49E-01 -7.29E-02
GWP-luluc kg CO 2 eq 1.3E-01 3.12E-02 1.85E-02 2.58E-06 1.33E-03 6.44E-04 1.66E-03 -1.52E-02
ODP kg CFC11 eq 5.7E-06 4.87E-16 6.46E-11 4.36E-17 2.07E-17 9.46E-09 1.51E-15 -1.13E-13
AP mol H+ eq 8.3E-01 1.23E-02 3.94E-02 3.79E-06 5.21E-04 5.07E-03 2.98E-03 -1.44E-01
EP-freshwater kg P eq 1.49E-02 1.13E-05 1.36E-04 4.88E-09 4.8E-07 2.34E-05 7.49E-06 -2.54E-05
EP-marine kg N eq 1.54E-01 5.66E-03 1.25E-02 9E-07 2.4E-04 1.78E-03 8.42E-04 -3.14E-02
EP-terrestrial mol N eq 1.75E+00 6.32E-02 1.27E-01 9.44E-06 2.69E-03 2.45E-02 9.14E-03 -3.48E-01
kg NMVOC
POCP 4.68E-01 1.1E-02 3.41E-02 2.44E-06 4.69E-04 4.84E-03 2.62E-03 -8.23E-02
eq
ADPE kg Sb eq 2.55E-03 2.9E-07 3.88E-06 5.35E-10 1.23E-08 3.37E-07 4.24E-08 -2.4E-05
ADPF MJ 2.81E+03 5.07E+01 2.03E+02 3.24E-02 2.15E+00 8.94E+00 6.42E+00 -5.18E+02
m3 world eq
WDP 2.05E+01 3.31E-02 1.25E+00 2.92E-04 1.41E-03 2.83E+00 4.08E-02 -2.65E+00
deprived
GWP = Global warming potential; ODP = Depletion potential of the stratospheric ozone layer; AP = Acidification potential of land and water; EP =
Eutrophication potential; POCP = Formation potential of tropospheric ozone photochemical oxidants; ADPE = Abiotic depletion potential for non-fossil
resources; ADPF = Abiotic depletion potential for fossil resources; WDP = Water (user) deprivation potential)
RESULTS OF THE LCA - INDICATORS TO DESCRIBE RESOURCE USE according to EN 15804+A2: 1 m2 Roof windows with
triple glazing
Parameter Unit A1 A2 A3 C1 C2 C3 C4 D
PERE MJ 2.77E+02 2.83E+00 1.04E+02 1.49E-02 1.2E-01 1.15E+02 7.39E-01 -9.69E+01
PERM MJ 1.22E+02 0 6.21E+01 0 0 -1.14E+02 0 0
PERT MJ 3.99E+02 2.83E+00 1.66E+02 1.49E-02 1.2E-01 1.68E+00 7.39E-01 -9.69E+01
PENRE MJ 2.56E+03 5.08E+01 1.89E+02 3.24E-02 2.16E+00 1.48E+02 6.42E+00 -5.2E+02
PENRM MJ 2.52E+02 0 1.44E+01 0 0 -1.4E+02 0 0
PENRT MJ 2.81E+03 5.08E+01 2.03E+02 3.24E-02 2.16E+00 8.95E+00 6.42E+00 -5.2E+02
SM kg 7.49E+00 0 1.37E-03 0 0 0 0 0
RSF MJ 0 0 0 0 0 0 0 0
NRSF MJ 0 0 0 0 0 0 0 0
FW m3 9.22E-01 3.24E-03 7.95E-02 1.45E-05 1.38E-04 6.67E-02 1.29E-03 -2.08E-01
PERE = Use of renewable primary energy excluding renewable primary energy resources used as raw materials; PERM = Use of renewable primary
energy resources used as raw materials; PERT = Total use of renewable primary energy resources; PENRE = Use of non-renewable primary energy
excluding non-renewable primary energy resources used as raw materials; PENRM = Use of non-renewable primary energy resources used as raw
materials; PENRT = Total use of non-renewable primary energy resources; SM = Use of secondary material; RSF = Use of renewable secondary fuels;
NRSF = Use of non-renewable secondary fuels; FW = Use of net fresh water
RESULTS OF THE LCA – WASTE CATEGORIES AND OUTPUT FLOWS according to EN 15804+A2:
1 m2 Roof windows with triple glazing
Parameter Unit A1 A2 A3 C1 C2 C3 C4 D
HWD kg 4.71E-03 2.56E-09 2.73E-04 8.56E-12 1.09E-10 1.45E-09 6.88E-10 -6.46E-08
NHWD kg 5.94E+00 7.54E-03 5.03E-01 2.3E-05 3.2E-04 2.57E+01 2.39E+01 -3.63E+00
RWD kg 4.02E-02 6.14E-05 1.61E-02 4.82E-06 2.61E-06 3.5E-04 5.94E-05 -2.25E-02
CRU kg 0 0 0 0 0 0 0 0
MFR kg 3.52E-02 0 2E+00 0 0 2E+01 0 0
MER kg 0 0 0 0 0 1.27E+01 0 0
EEE MJ 5.38E-02 0 0 0 0 0 0 4.99E+01
EET MJ 7.85E-02 0 0 0 0 0 0 9.07E+01
5 Environmental Product Declaration - VELUX Group - VELUX PUR roof windows (62 triple glazing configuration)
HWD = Hazardous waste disposed; NHWD = Non-hazardous waste disposed; RWD = Radioactive waste disposed; CRU = Components for re-use;
MFR = Materials for recycling; MER = Materials for energy recovery; EEE = Exported electrical energy; EET = Exported thermal energy
RESULTS OF THE LCA – additional impact categories according to EN 15804+A2-optional:
1 m2 Roof windows with triple glazing
Parameter Unit A1 A2 A3 C1 C2 C3 C4 D
Disease
PM 9.24E-06 6.62E-08 4.5E-07 3.19E-11 2.81E-09 4.05E-08 3.47E-08 -1.37E-06
incidence
IR kBq U235 eq 1.12E+01 8.79E-03 1.9E+00 7.91E-04 3.74E-04 6.21E-02 6.64E-03 -4.08E+00
ETP-fw CTUe 3.97E+03 3.66E+01 1.22E+02 1.36E-02 1.56E+00 5.36E+00 4.28E+00 -2.34E+02
HTP-c CTUh 1.26E-06 7.39E-10 6.14E-09 3.86E-13 3.14E-11 3.06E-10 4.4E-10 -2.78E-08
HTP-nc CTUh 3.4E-06 4.35E-08 5.52E-07 1.45E-11 1.85E-09 2.31E-08 4.78E-08 -3.21E-07
SQP SQP 1.69E+03 1.74E+01 8.34E+02 1.02E-02 7.4E-01 3.37E+00 1.32E+00 -3.59E+01
PM = Potential incidence of disease due to PM emissions; IR = Potential Human exposure efficiency relative to U235; ETP-fw = Potential comparative
Toxic Unit for ecosystems; HTP-c = Potential comparative Toxic Unit for humans (cancerogenic); HTP-nc = Potential comparative Toxic Unit for humans
(not cancerogenic); SQP = Potential soil quality index
Disclaimer 1 – for the indicator IRP. This impact category deals mainly with the eventual impact of low dose ionizing radiation on human
health of the nuclear fuel cycle. It does not consider effects due to possible nuclear accidents, occupational exposure or radioactive
waste disposal in underground facilities. Potential ionizing radiation from the soil, radon and (from) some construction materials is also
not measured by this indicator.
Disclaimer 2 – for the indicators ADPE, ADPF, WDP, ETP-fw, HTP-c, HTP-nc, SQP. The results of this environmental impact indicator
shall be used with care as the uncertainties on these results are high or as there is limited experience with the indicator.
References
IBU PCR Part A
IBU PCR Part A: Institut Bauen und Umwelt e.V., Product EN 15804
Category Rules for Building-Related Products and Services. EN 15804+A2+AC:2021, Sustainability of construction works -
Calculation Rules for the Life Cycle Assessment and Environmental Product Declarations - Core rules for the product
Requirements on the Project Report according to EN category of construction products.
15804+A2:2019.
EN 17213
IBU PCR Part B EN 17213:2020, Windows and doors – Environmental Product
IBU PCR Part B: Institut Bauen und Umwelt e.V., Requirements Declarations – Product category rules for windows and
on the EPD for Windows and doors, version 1.4: 2021. pedestrian doorsets.
IBU 2021 Candidate list
IBU 2021 Institut Bauen und Umwelt e.V.: General Instructions ECHA Candidate list of substances of very high concern, status
for the EPD programme of Institut Bauen und Umwelt e.V. 07.03.2022.
Version 2.0, Berlin: Institut Bauen und Umwelt e.V., 2021.
www.ibu-epd.com. ISO 10077-1
ISO 10077-1:2017, Thermal performance of windows, doors
EN 13501-1 and shutters - Calculation of thermal transmittance - Part 1:
EN 13501-1 EN13501-1, 2018: Fire classification of General.
construction products and building elements - Part 1:
Classification using data from reaction to fire tests. ISO 10077-2
ISO 10077-2:2017, Thermal performance of windows, doors
ISO 14025 and shutters - Calculation of thermal transmittance - Part 2:
DIN EN ISO 14025:2011-10, Environmental labels and Numerical method for frames.
declarations - Type III environmental declarations - Principles
and procedures. GaBi LCA software and database
The LCA modelling software is GaBi program version 9.5.2.49
EN 14351-1 with corresponding databases from Sphera Solutions GmbH.
EN 14351-1:2006+A2:2016, Windows and doors - Product Documentation hyperlink www.gabi-software.com/support/gabi.
standard, performance characteristics - Part 1:
Windows and external pedestrian doorsets.
6 Environmental Product Declaration - VELUX Group - VELUX PUR roof windows (62 triple glazing configuration)
Publisher
Institut Bauen und Umwelt e.V. +49 (0)30 3087748- 0
Hegelplatz 1 info@ibu-epd.com
10117 Berlin www.ibu-epd.com
Germany
Programme holder
Institut Bauen und Umwelt e.V. +49 (0)30 3087748- 0
Hegelplatz 1 info@ibu-epd.com
10117 Berlin www.ibu-epd.com
Germany
Author of the Life Cycle Assessment
FORCE Technology +4543250856
Park Alle 345 chme@force.dk
2605 Brøndby www.forcetechnology.com
Denmark
Owner of the Declaration
VELUX Group +4545164726
Ådalsvej 99 jakob.roerbech@velux.com
2970 Hørsholm www.velux.com
Denmark
7 Environmental Product Declaration - VELUX Group - VELUX PUR roof windows (62 triple glazing configuration)
