ENVIRONMENTAL PRODUCT DECLARATION
as per ISO 14025 and EN 15804+A2
Owner of the Declaration dormakaba International Holding GmbH
Publisher Institut Bauen und Umwelt e.V. (IBU)
Programme holder Institut Bauen und Umwelt e.V. (IBU)
Declaration number EPD-DOR-20220340-CBA2-EN
Issue date 11.09.2023
Valid to 14.03.2028
Optical Turnstile SU5000
dormakaba
www.ibu-epd.com | https://epd-online.com
General Information
dormakaba Optical Turnstile SU5000
Programme holder Owner of the declaration
IBU – Institut Bauen und Umwelt e.V. dormakaba International Holding GmbH
Hegelplatz 1 DORMA Platz 1
10117 Berlin 58256 Ennepetal
Germany Germany
Declaration number Declared product / declared unit
EPD-DOR-20220340-CBA2-EN 1 piece of the product: SU5000, consisting of the following items:
• housing
• steering
• drive unit
• panels
• sensors
• power adapter
• product packaging
This declaration is based on the product category rules: Scope:
Electronic and physical Access Control Systems, 01.08.2021 This Environmental Product Declaration refers to a specific Optical
(PCR checked and approved by the SVR) Turnstile manufactured by dormakaba. The production site is located in
Chino (USA).
Issue date The data represents the year 2022.
The owner of the declaration shall be liable for the underlying information
11.09.2023
and evidence; the IBU shall not be liable with respect to manufacturer
information, life cycle assessment data and evidences.
Valid to
The EPD was created according to the specifications of EN 15804+A2. In
14.03.2028 the following, the standard will be simplified as EN 15804.
Verification
The standard EN 15804 serves as the core PCR
Independent verification of the declaration and data according to ISO
14025:2011
internally X externally
Dipl.-Ing. Hans Peters
(Chairman of Institut Bauen und Umwelt e.V.)
Florian Pronold Dr.-Ing. Wolfram Trinius,
(Managing Director Institut Bauen und Umwelt e.V.) (Independent verifier)
1 Environmental Product Declaration - dormakaba - Optical Turnstile SU5000
Product
Performance data of the product with respect to its
Product description/Product definition characteristics in accordance with the relevant technical
The Optical Turnstile SU5000 has a slim size. It is the ideal provision which can be applied are mentioned above.
solution for areas where space is limited. The turnstile allows
bi-directional passage when the product solution is integrated in Base materials/Ancillary materials
the building's access control system. The system offers many The major material composition including the packaging of the
different operational modes and features to suit a variety of product is listed below:
applications. Name Value Unit
Steel 46 %
For the SU 5000 the standards which can be applied are the
Plastics 25 %
following:
Plexi Glass 17 %
• UL2593
Aluminium 6 %
• 2011/65/EU (RoHS)
Electronics 4 %
The CE marking takes into account the proof of conformity with Zinc 2 %
the respective harmonised standards based on the legal
The product includes partial articles which contain substances
provisions above.
listed in the Candidate List of REACH Regulation
Application 1907/2006/EC (date: 14.06.2023) exceeding 0.1 percentage by
mass: no
SU5000 is ideal for secured entry control applications for main
lobby access, employee entrances, elevator bank access and
The Candidate List can be found on the ECHA website
visitor management applications. Areas of application are:
address: https:echa.europa.eu/de/home.
• Corporate security
• Industrial facilities Reference service life
• Goverment security The reference service life of the Optical Turnstile SU 5000
• Higher education amounts to 20 years, depending on the application and
• Health and fitness frequency of use. For repairs and renewals, suitable spare
parts are available. The Optical Turnstile is tested and certified
Technical Data
to UL 2593.
The Optical Turnstile SU 5000 has following technical
properties:
Name Value Unit
Length 1321 mm
Height 1038 mm
Width 993 mm
Passage way 711 mm
LCA: Calculation rules
Declared Unit Construction stage - Modules A4-A5
The declared unit is 1 piece of the product: Optical Turnstile The construction process stage includes:
SU5000 including packaging. — A4, transport to the building site;
Declared unit — A5, installation into the building;
including provision of all materials, products and energy, as well
Name Value Unit
as waste processing up to the end-of-waste state or disposal of
Declared unit 1 pce.
final residues during the construction process stage.
Mass (total system) 166.47 kg
Maintenance
System boundary – Module B2
The type of EPD is: cradle to gate with options, modules C1– This module includes the production and
C4, and module D (A1–A3 + C + D and additional modules: A4 the end of life of the batteries. The
+ A5 + B6) potential use of batteries is declared in module B2.
Production - Module A1-A3 Use stage - Module B6
The product stage includes: The use stage related to the operation of the building includes:
— A1, raw material extraction, processing and mechanical — B6, operational energy use
treatments, processing of secondary material input (e.g. The potential use of electricity from the grid is declared in
recycling processes), module B6.
— A2, transport to the manufacturer,
— A3, manufacturing and assembly including provision of all End-of-life stage– Modules C1-C4 and D
materials, products and energy, as well as waste processing up The end-of-life stage includes:
to the end-of waste state. — C1, de-construction, demolition:
2 Environmental Product Declaration - dormakaba - Optical Turnstile SU5000
— C2, transport to waste processing; Land or region, in which the declared product system is
— C3, waste processing for reuse, recovery and/or recycling; manufactured, used or handled at the end of the product´s
— C4, disposal; lifespan: United States
including provision and all transport, provision of all materials,
products and related energy and water use.
Comparability
Module D (Benefits and loads beyond the system boundary)
includes: Basically, a comparison or an evaluation of EPD data is only
— D, recycling potentials, expressed as net impacts and possible if all the data sets to be compared were created
benefits. according to EN 15804 and the building context, respectively
the product-specific characteristics of performance, are taken
Geographic Representativeness into account. GaBi, SP40.
LCA: Scenarios and additional technical information
Characteristic product properties of biogenic carbon
Information on describing the biogenic Carbon Content at Operational energy use (B6)
factory gate
Name Value Unit
Name ValueUnit
Electricity consumption for 1 year 183.23 kW
kg
Biogenic carbon content in product - Days per year in use 365 days
C
On mode per day 1,1 h
Biogenic carbon content in accompanying kg
0,425 Idle mode per day 22,9 h
packaging C
On mode power 40 W
Idle mode power 20 W
End of life (C1-C4)
Transport to the building site (A4) C1: The product expansion depends on the building. The
Name Value Unit product share is so low that no environmental burden is
assumed.
Litres of fuel 0.00276 l/100km
C2: Transport to waste management is 50 km.
Capacity utilisation (including empty runs) 55 %
Name Value Unit
Transport distance 100 km
Collected separately waste type 164.97 kg
The product is transported via truck. The main distribution
Recycling 91.1 kg
region is North America. In order to allow scaling to a specific
Energy recovery 68.6 kg
point of installation 100 km are declared.
Landfilling 5.27 kg
Installation into the building (A5) The product is disassembled in a recycling process.
Material recycling is then assumed for the metals, electronic
Name Value Unit
and electromechanics. The plastic components are assumed to
Paper packaging 1,1531 kg
be incinerated with energy recovery. Minor proportions of
Plastic packaging 0,393 kg residues arising from the recycling process are landfilled.
Region for the End of Life is: Global.
Reference service life
Name Value Unit
Life Span according to the manufacturer 20 a
3 Environmental Product Declaration - dormakaba - Optical Turnstile SU5000
LCA: Results
B2 declares the environmental impact for the use stage under the assumption that batteries are used.
B6 declares the environmental impact for the use stage under the assumption that electricity from the grid (B6/1: region EU, B6/2:
region mainly US) is used.
DESCRIPTION OF THE SYSTEM BOUNDARY (X = INCLUDED IN LCA; MND = MODULE OR INDICATOR NOT DECLARED; MNR
= MODULE NOT RELEVANT)
Benefits and
Construction loads beyond
Product stage Use stage End of life stage
process stage the system
boundaries
la ire ta m w a Ry lp p u s tro p s n a rT g n iru tc a fu n a M e h t m o rf tro p s n a rTe tis e h t o t e ta g y lb m e s s A e s U e c n a n e tn ia M ria p e R tn e m e c a lp e R tn e m h s ib ru fe R y g re n e la n o ita re p Oe s u re ta w la n o ita re p Oe s u n o itc u rts n o c -e Dn o itilo m e d tro p s n a rT g n is s e c o rp e ts a W la s o p s iD -e s u e R-y re v o c e R-g n ilc y c e Rla itn e to p
A1 A2 A3 A4 A5 B1 B2 B3 B4 B5 B6 B7 C1 C2 C3 C4 D
X X X X X MND MND MNR MNR MNR X MND X X X X X
RESULTS OF THE LCA - ENVIRONMENTAL IMPACT according to EN 15804+A2: 1 piece SU5000 Optical Turnstile with
Motorized Barriers
Parameter Unit A1-A3 A4 A5 B6 C1 C2 C3 C4 D
GWP-total kg CO 2 eq 8.21E+02 1.46E+00 2.63E+00 2.06E+03 0 7.15E-01 1.74E+02 8E-02 -4.36E+02
GWP-fossil kg CO 2 eq 8.2E+02 1.39E+00 1.04E+00 2.06E+03 0 6.83E-01 1.74E+02 8E-02 -4.36E+02
GWP-biogenic kg CO 2 eq -4.19E-01 6.4E-02 1.59E+00 4.45E-01 0 3.2E-02 9E-03 2.73E-04 8.94E-01
GWP-luluc kg CO 2 eq 8.94E-01 3.31E-05 8.34E-05 6.21E-01 0 1.63E-05 1E-02 2.3E-04 -5.87E-01
ODP kg CFC11 eq 1.92E-09 1.47E-16 7.98E-16 7.25E-12 0 7.21E-17 8.79E-14 2.96E-16 -4.98E-10
AP mol H+ eq 3.81E+00 1E-03 6.36E-04 3.33E+00 0 6.84E-04 3.1E-02 5.73E-04 -1.72E+00
EP-freshwater kg P eq 1.07E-03 2.98E-07 1.38E-07 1E-03 0 1.46E-07 1.4E-05 1.37E-07 -3.92E-04
EP-marine kg N eq 5.38E-01 4.43E-04 2.05E-04 7.13E-01 0 2.18E-04 7E-03 1.48E-04 -2.69E-01
EP-terrestrial mol N eq 5.86E+00 5E-03 3E-03 7.65E+00 0 2E-03 1.41E-01 2E-03 -2.92E+00
kg NMVOC
POCP 2.59E+00 1E-03 5.49E-04 2.04E+00 0 6.15E-04 1.9E-02 4.47E-04 -8.11E-01
eq
ADPE kg Sb eq 4.35E-02 4.17E-08 1.16E-08 4.09E-04 0 2.05E-08 1.21E-06 7.18E-09 -1.9E-02
ADPF MJ 1.35E+04 1.97E+01 9.79E-01 3.33E+04 0 9.69E+00 8.08E+01 1.05E+00 -5.8E+03
m3 world eq
WDP 1.71E+02 3E-03 3.05E-01 3.98E+02 0 1E-03 1.78E+01 8E-03 -1.22E+02
deprived
GWP = Global warming potential; ODP = Depletion potential of the stratospheric ozone layer; AP = Acidification potential of land and water; EP =
Eutrophication potential; POCP = Formation potential of tropospheric ozone photochemical oxidants; ADPE = Abiotic depletion potential for non-fossil
resources; ADPF = Abiotic depletion potential for fossil resources; WDP = Water (user) deprivation potential)
RESULTS OF THE LCA - INDICATORS TO DESCRIBE RESOURCE USE according to EN 15804+A2: 1 piece SU5000 Optical
Turnstile with Motorized Barriers
Parameter Unit A1-A3 A4 A5 B6 C1 C2 C3 C4 D
PERE MJ 2.1E+03 6.2E-02 1.41E+01 5.27E+03 0 3.1E-02 2.1E+01 1.37E-01 -1.4E+03
PERM MJ 1.39E+01 0 -1.38E+01 0 0 0 -3E-02 0 0
PERT MJ 2.11E+03 6.2E-02 2.14E-01 5.27E+03 0 3.1E-02 2.1E+01 1.37E-01 -1.4E+03
PENRE MJ 1.12E+04 1.98E+01 1.79E+01 3.33E+04 0 9.7E+00 2.37E+03 1.05E+00 -5.8E+03
PENRM MJ 2.31E+03 0 -1.69E+01 0 0 0 -2.29E+03 0 0
PENRT MJ 1.35E+04 1.98E+01 9.79E-01 3.33E+04 0 9.7E+00 8.08E+01 1.05E+00 -5.8E+03
SM kg 3.82E+01 0 0 0 0 0 0 0 0
RSF MJ 0 0 0 0 0 0 0 0 0
NRSF MJ 0 0 0 0 0 0 0 0 0
FW m3 7.51E+00 1.12E-04 7E-03 1.22E+01 0 5.48E-05 4.26E-01 2.64E-04 -5.39E+00
PERE = Use of renewable primary energy excluding renewable primary energy resources used as raw materials; PERM = Use of renewable primary
energy resources used as raw materials; PERT = Total use of renewable primary energy resources; PENRE = Use of non-renewable primary energy
excluding non-renewable primary energy resources used as raw materials; PENRM = Use of non-renewable primary energy resources used as raw
materials; PENRT = Total use of non-renewable primary energy resources; SM = Use of secondary material; RSF = Use of renewable secondary fuels;
NRSF = Use of non-renewable secondary fuels; FW = Use of net fresh water
RESULTS OF THE LCA – WASTE CATEGORIES AND OUTPUT FLOWS according to EN 15804+A2:
1 piece SU5000 Optical Turnstile with Motorized Barriers
Parameter Unit A1-A3 A4 A5 B6 C1 C2 C3 C4 D
HWD kg 4.32E-05 1.92E-09 2.53E-09 1.28E-05 0 9.41E-10 3.08E-07 1.6E-08 -1.89E-05
NHWD kg 7.67E+01 2E-03 1.55E-01 1.03E+01 0 9.92E-04 1.81E+01 5.27E+00 -4.15E+01
RWD kg 2.59E-01 2.12E-05 4.43E-05 2.97E+00 0 1.04E-05 3E-03 1.19E-05 -2.18E-01
CRU kg 0 0 0 0 0 0 0 0 0
MFR kg 0 0 0 0 0 0 8.96E+01 0 0
4 Environmental Product Declaration - dormakaba - Optical Turnstile SU5000
MER kg 0 0 0 0 0 0 0 0 0
EEE MJ 9.74E-01 0 4.32E+00 0 0 0 0 0 0
EET MJ 1.77E+00 0 8.73E+00 0 0 0 0 0 0
HWD = Hazardous waste disposed; NHWD = Non-hazardous waste disposed; RWD = Radioactive waste disposed; CRU = Components for re-use;
MFR = Materials for recycling; MER = Materials for energy recovery; EEE = Exported electrical energy; EET = Exported thermal energy
RESULTS OF THE LCA – additional impact categories according to EN 15804+A2-optional:
1 piece SU5000 Optical Turnstile with Motorized Barriers
Parameter Unit A1-A3 A4 A5 B6 C1 C2 C3 C4 D
Disease
PM 5.35E-05 7.32E-09 4.81E-09 2.98E-05 0 3.59E-09 3.96E-07 7.1E-09 -3.04E-05
incidence
IR kBq U235 eq 3.35E+01 3E-03 6E-03 2.45E+02 0 1E-03 2.7E-01 1E-03 -3.83E+01
ETP-fw CTUe 6.11E+03 1.4E+01 4.19E-01 9.93E+03 0 6.87E+00 3.03E+01 5.99E-01 -2.37E+03
HTP-c CTUh 9.15E-05 2.63E-10 2.8E-11 2.14E-07 0 1.29E-10 2.62E-09 8.88E-11 -5.36E-07
HTP-nc CTUh 2.47E-05 1.13E-08 2.09E-09 8.08E-06 0 5.52E-09 2.66E-07 9.78E-09 2.14E-06
SQP SQP 2.23E+03 5.1E-02 2.76E-01 3.05E+03 0 2.5E-02 2.42E+01 2.19E-01 -7.01E+02
PM = Potential incidence of disease due to PM emissions; IR = Potential Human exposure efficiency relative to U235; ETP-fw = Potential comparative
Toxic Unit for ecosystems; HTP-c = Potential comparative Toxic Unit for humans (cancerogenic); HTP-nc = Potential comparative Toxic Unit for humans
(not cancerogenic); SQP = Potential soil quality index
Disclaimer 1 – for the indicator “Potential Human exposure efficiency relative to U235”. This impact category deals mainly with the
eventual impact of low-dose ionizing radiation on human health of the nuclear fuel cycle. It does not consider effects due to possible
nuclear accidents, occupational exposure or radioactive waste disposal in underground facilities. Potential ionizing radiation from the
soil, radon and from some construction materials is also not measured by this indicator.
Disclaimer 2 – for the indicators “abiotic depletion potential for non-fossil resources”, “abiotic depletion potential for fossil resources”,
“water (user) deprivation potential, deprivation-weighted water consumption”, “potential comparative toxic unit for ecosystems”,
“potential comparative toxic unit for humans – cancerogenic”, “Potential comparative toxic unit for humans - not cancerogenic”,
“potential soil quality index”. The results of this environmental impact indicator shall be used with care as the uncertainties on these
results are high as there is limited experience with the indicator.
References
ISO 14025 und Umwelt e.V. Version 2.0, Berlin: Institut Bauen und Umwelt
ISO 14025:2011-10, Environmental labels and declarations — e.V., 2021. www.ibu-epd.com
Type III environmental declarations - Principles and procedures.
GaBi ts software
EN 15804 Sphera Solutions GmbH Gabi Software System and Database
EN 15804:2019+A2 (in press), Sustainability of construction for Life Cycle Engineering 1992-2020 Version 10.0.0.71
works — Environmental Product Declarations — Core rules for University of Stuttgart Leinfelden-Echterdingen
the product category of construction products.
GaBi ts documentation
UL 2593 GaBi life cycle inventory data documentation (https://www.gabi-
UL 2593: 2011-26,Underwriters Laboratories, UL LLC Outline of software.com/support/gabi/gabidatabase-2020-lci-
Investigation for Motor Driven Turnstile Operators and Systems documentation/).
REACH LCA-tool dormakaba
Regulation (EC) No 1907/2006 of the European Parliament and Tool no.: IBU-DOR-202109-LT1-EN.
of the Council on the Registration, Evaluation, Authorisation Developed by Sphera Solutions GmbH.
and Restriction of Chemicals (REACH).
PCR Part A
RoHS PCR – Part A: Calculation Rules for the Life Cycle Assessment
Directive on the restriction of the use of certain hazardous and Requirements on the Project Re-port according to EN
substances in electrical and electronic equipment (RoHS), 15804+A2:2019, Version 1.0, Institut Bauen und Umwelt e.V.,
Directive (EU) No 2011/65. www.ibu-epd.com.
European Chemicals Agency (ECHA) PCR Part B
https://echa.europa.eu/de/ PCR – Part B: Requirements on the EPD for Electronic and
physical Access Control Systems, version 08/2021, Institut
Further References Bauen und Umwelt e.V., www.ibu-epd.com.
IBU 2021
General Instructions for the EPD programme of Institut Bauen
5 Environmental Product Declaration - dormakaba - Optical Turnstile SU5000
Publisher
Institut Bauen und Umwelt e.V. +49 (0)30 3087748- 0
Hegelplatz 1 info@ibu-epd.com
10117 Berlin www.ibu-epd.com
Germany
Programme holder
Institut Bauen und Umwelt e.V. +49 (0)30 3087748- 0
Hegelplatz 1 info@ibu-epd.com
10117 Berlin www.ibu-epd.com
Germany
Author of the Life Cycle Assessment
Sphera Solutions GmbH +49 711 341817-0
Hauptstraße 111- 113 info@sphera.com
70771 Leinfelden-Echterdingen www.sphera.com
Germany
Owner of the Declaration
dormakaba International Holding GmbH +49 2333 793-0
DORMA Platz 1 info.de@dormakaba.com
58256 Ennepetal www.dormakaba.com
Germany
6 Environmental Product Declaration - dormakaba - Optical Turnstile SU5000
