ENVIRONMENTAL PRODUCT DECLARATION
as per ISO 14025 and EN 15804+A2
Owner of the Declaration OGRO Beschlagtechnik GmbH
Publisher Institut Bauen und Umwelt e.V. (IBU)
Programme holder Institut Bauen und Umwelt e.V. (IBU)
Declaration number EPD-OGR-20240052-CBA5-EN
Issue date 18.06.2024
Valid to 17.06.2029
Aluminium lever and window handle CORE/PREMIUM
OGRO
www.ibu-epd.com | https://epd-online.com
General Information
OGRO Aluminium lever and window handle
CORE/PREMIUM
Programme holder Owner of the declaration
IBU – Institut Bauen und Umwelt e.V. OGRO Beschlagtechnik GmbH
Hegelplatz 1 Donnenberger Straße 2
10117 Berlin 42553 Velbert
Germany Germany
Declaration number Declared product / declared unit
EPD-OGR-20240052-CBA5-EN The declared unit is one (1 piece) aluminium lever handle from the OGRO
PREMIUM and CORE series, including packaging materials. The average
fitting including packaging weighs 763 g.
This declaration is based on the product category rules: Scope:
Building Hardware products, 01.08.2021 This Environmental Product Declaration refers to a specific aluminium
(PCR checked and approved by the SVR) lever handle manufactured by OGRO. The EPD is also representative for
aluminium window handles. The production site is located in Velbert
(Germany).
Issue date Data represents the year 2023.
18.06.2024
The owner of the declaration shall be liable for the underlying information
and evidence; the IBU shall not be liable with respect to manufacturer
information, life cycle assessment data and evidences.
Valid to
17.06.2029 The EPD was created according to the specifications of EN 15804+A2. In
the following, the standard will be simplified as EN 15804.
Verification
The standard EN 15804 serves as the core PCR
Independent verification of the declaration and data according to ISO
14025:2011
internally X externally
Dipl.-Ing. Hans Peters
(Chairman of Institut Bauen und Umwelt e.V.)
Florian Pronold Matthias Klingler,
(Managing Director Institut Bauen und Umwelt e.V.) (Independent verifier)
1 Environmental Product Declaration - OGRO - Aluminium lever and window handle CORE/PREMIUM
Product
• DIN 17440: Steel and steel alloys
Product description/Product definition
• EN 179: Locks and fittings
OGRO Beschlagtechnik GmbH manufactures door and window
• EN 1125: Locks and fittings
fittings made of stainless steel or aluminium for the premium
• EN 1634: Fire resistance and smoke control tests for
real estate market. This EPD declares OGRO Premium and
door and shutter assemblies
CORE lever and window handles made of aluminium.
• EN 1906: Requirements and test methods for lever
handles and knob furniture
For the placing the lever handles on the market in the
• EN 13126-3: Building hardware - Hardware for windows
European Union/European Free Trade Association (EU/EFTA)
and door height windows
(with the exception of Switzerland) the following legal provisions
• DIN 18082, Part 1: Fire protection barriers, steel doors T
apply:
30-1
• EN 179 • DIN 18095, Parts 1 + 2: Smoke control doors
• DIN 18255: Building hardware
For the placing the window handles on the market in the • DIN 18257: Security plates
European Union/European Free Trade Association (EU/EFTA) • DIN 18273: Lever handle units for fire doors and smoke
(with the exception of Switzerland) the following legal provisions control doors
apply: • DIN 4102, Parts 5 + 18: Fire behaviour of building
materials and building components
• EN 13126-3 • DIN 18040: Construction of accessible buildings
The CE-marking takes into account the proof of conformity with Performance data of the products with respect to its
the respective harmonized standards based on the legal characteristics in accordance with the relevanttechnical
provisions above. For the application and use the respective provision which can be applied arementioned above.
national provisions apply.
Base materials/Ancillary materials
The major material composition including the packaging of the
Application product is listed below:
The door and window handles are suitable for practically all • Aluminium: 58%
applications. • Steel: 24%
Lever handles: • Cardboard: 13%
• For use on doors which are subject to frequent force, • Plastics: 4%
e.g. football stadiums, military barracks, schools, public • Stainless steel: 1%
toilets
• For extremely high-traffic areas and intensive use in The lever and window handles include partial articles which
buildings contain substances listed in the Candidate List of REACH
• Use in public buildings, e.g. hospitals or administrative Regulation 1907/2006/EC (date: 14.06.2023) exceeding 0.1
buildings percentage bymass: yes
• Manifold barrier-free applications
• Use on glass doors • Lead (Pb): 7439-92-1 (CAS-No) is used in the steel
• Use on mechanically high-strength apartment entrance alloy. The concentration of lead in the alloy does not
doors with requirements incl. in accordance with DIN exceed 0,35% (by mass).
18257
• Use on panic, escape, rescue and fire safety doors The Candidate List can be found on the ECHA website
• Use on doors with electronic access control address: https:echa.europa.eu/de/home.
Window handles: Reference service life
The reference service life of the aluminium lever handles
• For use on wooden, plastic or aluminium profiles
amount to 40 years and depends on the application and
• For high-traffic areas and intensive use in buildings
frequency of use. For repairs or renewals, suitable spare parts
• Use in public buildings, e.g. hospitals or administrative
are available. The lever handles are tested according to EN
buildings
1906, meaning they are designed to withstand a minimum of
• Suitable for all standard window handle gears with
1.000.000 cycles. The reference service life of the aluminium
variable pin adjustment
window handles amount to 20 years and depends on the
• Simple operation with forces according to EN standards
application and frequency of use. For repairs or renewals,
Technical Data suitable spare parts are available. The window handles are
The aluminium lever and window handles comply with following tested according to EN 13126-3, meaning they are designed to
standards: withstand a minimum of 25.0000 cycles.
LCA: Calculation rules
Name Value Unit
Declared Unit
Declared unit 1 piece/product
The declared unit is 1 piece of the product: Aluminium lever and
Mass of declared Product excluding
window handle 0.667 kg
packaging
Packaging 0.098 kg
2 Environmental Product Declaration - OGRO - Aluminium lever and window handle CORE/PREMIUM
Other declared units are allowed if the conversion is shown residues during the construction process stage.
transparently.
End-of-life stage– Modules C1-C4 and D
The end-of-life stage includes:— C1, deconstruction,
System boundary
demolition:— C2, transport to waste processing;— C3, waste
The type of EPD is according to EN 15804: "cradle to processing for reuse, recovery and/or recycling;— C4, disposal;
gate with options, modules C1–C4, and module D".The including provision and all transport, provision of all materials,
following modules are declared: A1-A3, C1-C4, Dand additional products and related energy and water use. Module D (Benefits
modules: A4 + A5 and loads beyond the system boundary) includes:— D,
recycling potentials, expressed as net impacts and benefits.
Production - Module A1-A3
The product stage includes:— A1, raw material extraction, Geographic Representativeness
processing and mechanical treatments, processing of Land or region, in which the declared product system is
secondary material input (e.g. recycling processes),— A2, manufactured, used or handled at the end of the product´s
transport to the manufacturer,— A3, manufacturing and lifespan: Global
assembly including provision of all materials, products and
energy, as well as waste processing up to the end-of waste
state. Comparability
Basically, a comparison or an evaluation of EPD data is only
Construction stage - Modules A4-A5 possible if all the data sets to be compared were created
The construction process stage includes:— A4, transport to the according to EN 15804 and the building context, respectively
building site;— A5, installation into the building; including the product-specific characteristics of performance, are taken
provision of all materials, products and energy, as well as waste into account.
processing up to the end-of waste state or disposal of final Background database: GaBi ts, SP40, CUP 2020.1
LCA: Scenarios and additional technical information
Name ValueUnit
Characteristic product properties of biogenic carbon
Output substances following waste treatment on
0.098 kg
Information on describing the biogenic carbon content at site (packaging)
factory gate
Reference service life
Name ValueUnit
kg Name Value Unit
Biogenic carbon content in product -
C Reference service life 40 a
Biogenic carbon content in accompanying kg
0.04 End of life (C1-C4)
packaging C
C1: The product dismantling from the building is done manually
Note: 1 kg of biogenic carbon is equivalent to 44/12 kg of CO 2. without environmental burden.
C2: Transport to waste treatment at end of life is 50 km.
Name Value Unit
Collected separately waste type 0.667 kg
Transport to the building site (A4)
Recycling 0.638 kg
Name Value Unit Energy recovery 0.029 kg
Litres of fuel 0.00276 l/100km
Reuse, recovery and/or recycling potentials (D), relevant
Transport distance 100 km
scenario information
Capacity utilisation (including empty runs) 55 %
The collection rate is 100%.
Transport distance is declared for 100km by truck in order to
Name Value Unit
allow scaling to a specific point of installation.
Recycling 100 %
Installation into the building (A5)
3 Environmental Product Declaration - OGRO - Aluminium lever and window handle CORE/PREMIUM
LCA: Results
DESCRIPTION OF THE SYSTEM BOUNDARY (X = INCLUDED IN LCA; MND = MODULE OR INDICATOR NOT DECLARED; MNR
= MODULE NOT RELEVANT)
Benefits and
Construction loads beyond
Product stage Use stage End of life stage
process stage the system
boundaries
la ire ta m w a Ry lp p u s tro p s n a rT g n iru tc a fu n a M e h t m o rf tro p s n a rTe tis e h t o t e ta g y lb m e s s A e s U e c n a n e tn ia M ria p e R tn e m e c a lp e R tn e m h s ib ru fe R y g re n e la n o ita re p Oe s u re ta w la n o ita re p Oe s u n o itc u rts n o c -e Dn o itilo m e d tro p s n a rT g n is s e c o rp e ts a W la s o p s iD -e s u e R-y re v o c e R-g n ilc y c e Rla itn e to p
A1 A2 A3 A4 A5 B1 B2 B3 B4 B5 B6 B7 C1 C2 C3 C4 D
X X X X X MND MND MNR MNR MNR MND MND X X X X X
RESULTS OF THE LCA - ENVIRONMENTAL IMPACT according to EN 15804+A2: 1 piece
Parameter Unit A1-A3 A4 A5 C1 C2 C3 C4 D
GWP-total kg CO 2 eq 7.89E+00 7E-03 1.39E-01 0 3E-03 7.9E-02 0 -2.83E+00
GWP-fossil kg CO 2 eq 8E+00 6E-03 3E-03 0 3E-03 7.9E-02 0 -2.82E+00
GWP-biogenic kg CO 2 eq -1.26E-01 2.96E-04 1.35E-01 0 1.29E-04 1.84E-06 0 -9E-03
GWP-luluc kg CO 2 eq 1E-02 1.52E-07 2.29E-06 0 6.64E-08 4.45E-06 0 -5.13E-04
ODP kg CFC11 eq 1.19E-12 6.75E-19 2.5E-17 0 2.94E-19 3.97E-17 0 -2.27E-11
AP mol H+ eq 2.8E-02 6.4E-06 3.89E-05 0 2.79E-06 1.4E-05 0 -1.1E-02
EP-freshwater kg P eq 1.83E-05 1.37E-09 4.9E-09 0 5.97E-10 6.34E-09 0 -1.45E-06
EP-marine kg N eq 5.01E-03 2.04E-06 1.41E-05 0 8.88E-07 3.16E-06 0 -1E-03
EP-terrestrial mol N eq 5.01E-02 2.26E-05 1.75E-04 0 9.87E-06 6.39E-05 0 -1.5E-02
kg NMVOC
POCP 1.3E-02 5.76E-06 3.72E-05 0 2.51E-06 8.75E-06 0 -4E-03
eq
ADPE kg Sb eq 1.6E-05 1.92E-10 3.96E-10 0 8.36E-11 5.45E-10 0 -1.72E-06
ADPF MJ 1.01E+02 9.1E-02 4.4E-02 0 4E-02 3.7E-02 0 -4.08E+01
m3 world eq
WDP 8.35E-01 1.25E-05 1.7E-02 0 5.46E-06 8E-03 0 -1.36E-01
deprived
GWP = Global warming potential; ODP = Depletion potential of the stratospheric ozone layer; AP = Acidification potential of land and water; EP =
Eutrophication potential; POCP = Formation potential of tropospheric ozone photochemical oxidants; ADPE = Abiotic depletion potential for non-fossil
resources; ADPF = Abiotic depletion potential for fossil resources; WDP = Water (user) deprivation potential)
RESULTS OF THE LCA - INDICATORS TO DESCRIBE RESOURCE USE according to EN 15804+A2: 1 piece
Parameter Unit A1-A3 A4 A5 C1 C2 C3 C4 D
PERE MJ 4.69E+01 2.86E-04 1.18E+00 0 1.25E-04 9E-03 0 -1.95E+01
PERM MJ 1.18E+00 0 -1.18E+00 0 0 0 0 0
PERT MJ 4.81E+01 2.86E-04 8E-03 0 1.25E-04 9E-03 0 -1.95E+01
PENRE MJ 1E+02 9.1E-02 4.4E-02 0 4E-02 4.99E-01 0 -4.08E+01
PENRM MJ 4.62E-01 0 0 0 0 -4.62E-01 0 0
PENRT MJ 1.01E+02 9.1E-02 4.4E-02 0 4E-02 3.7E-02 0 -4.08E+01
SM kg 2.05E-01 0 0 0 0 0 0 0
RSF MJ 0 0 0 0 0 0 0 0
NRSF MJ 0 0 0 0 0 0 0 0
FW m3 7.1E-02 5.13E-07 4.06E-04 0 2.24E-07 1.93E-04 0 -3.4E-02
PERE = Use of renewable primary energy excluding renewable primary energy resources used as raw materials; PERM = Use of renewable primary
energy resources used as raw materials; PERT = Total use of renewable primary energy resources; PENRE = Use of non-renewable primary energy
excluding non-renewable primary energy resources used as raw materials; PENRM = Use of non-renewable primary energy resources used as raw
materials; PENRT = Total use of non-renewable primary energy resources; SM = Use of secondary material; RSF = Use of renewable secondary fuels;
NRSF = Use of non-renewable secondary fuels; FW = Use of net fresh water
RESULTS OF THE LCA – WASTE CATEGORIES AND OUTPUT FLOWS according to EN 15804+A2:
1 piece
Parameter Unit A1-A3 A4 A5 C1 C2 C3 C4 D
HWD kg 1.03E-07 8.81E-12 6.47E-11 0 3.84E-12 1.39E-10 0 -1.75E-08
NHWD kg 1.22E+00 9.28E-06 4E-03 0 4.05E-06 8E-03 0 -7.6E-01
RWD kg 7E-03 9.74E-08 2.31E-06 0 4.25E-08 1.36E-06 0 -5E-03
CRU kg 0 0 0 0 0 0 0 0
MFR kg 0 0 0 0 0 6.36E-01 0 0
MER kg 0 0 0 0 0 0 0 0
EEE MJ 0 0 2.1E-01 0 0 1.46E-01 0 0
EET MJ 0 0 3.81E-01 0 0 3.35E-01 0 0
HWD = Hazardous waste disposed; NHWD = Non-hazardous waste disposed; RWD = Radioactive waste disposed; CRU = Components for re-use;
MFR = Materials for recycling; MER = Materials for energy recovery; EEE = Exported electrical energy; EET = Exported thermal energy
4 Environmental Product Declaration - OGRO - Aluminium lever and window handle CORE/PREMIUM
RESULTS OF THE LCA – additional impact categories according to EN 15804+A2-optional:
1 piece
Parameter Unit A1-A3 A4 A5 C1 C2 C3 C4 D
Disease
PM 3.64E-07 3.37E-11 2.16E-10 0 1.47E-11 1.79E-10 0 -1.74E-07
incidence
IR kBq U235 eq 9.51E-01 1.39E-05 3.57E-04 0 6.07E-06 1.22E-04 0 -9.35E-01
ETP-fw CTUe 3.6E+01 6.4E-02 2.1E-02 0 2.8E-02 1.4E-02 0 -1.55E+01
HTP-c CTUh 1.3E-08 1.21E-12 1.1E-12 0 5.27E-13 1.19E-12 0 -8.11E-10
HTP-nc CTUh 7.92E-08 5.17E-11 4.77E-11 0 2.25E-11 1.2E-10 0 -2.02E-08
SQP SQP 4.17E+01 2.33E-04 1.2E-02 0 1.02E-04 1.1E-02 0 -1.32E+00
PM = Potential incidence of disease due to PM emissions; IR = Potential Human exposure efficiency relative to U235; ETP-fw = Potential comparative
Toxic Unit for ecosystems; HTP-c = Potential comparative Toxic Unit for humans (cancerogenic); HTP-nc = Potential comparative Toxic Unit for humans
(not cancerogenic); SQP = Potential soil quality index
Disclaimer 1 – for the indicator “Potential Human exposure efficiency relative to U235”. This impact category deals mainly with the
eventual impact of low-dose ionizing radiation on human health of the nuclear fuel cycle. It does not consider effects due to possible
nuclear accidents, occupational exposure or radioactive waste disposal in underground facilities. Potential ionizing radiation from the
soil, radon and from some construction materials is also not measured by this indicator.
Disclaimer 2 – for the indicators “abiotic depletion potential for non-fossil resources”, “abiotic depletion potential for fossil resources”,
“water (user) deprivation potential, deprivation-weighted water consumption”, “potential comparative toxic unit for ecosystems”,
“potential comparative toxic unit for humans – cancerogenic”, “Potential comparative toxic unit for humans - not cancerogenic”,
“potential soil quality index”. The results of this environmental impact indicator shall be used with care as the uncertainties on these
results are high as there is limited experience with the indicator.
This EPD was created using a software tool.
References
EN 15804 PCR – Part B: Requirements on the EPD for Building Hardware
EN 15804+A2:2019+AC:2021, Sustainability of construction product, version 1.2, Institut Bauen und Umwelt e.V., www.ibu-
works - Environmental Product Declarations - Core rules for the epd.com, 2017
product category of construction products
EN 10088
ISO 14025 EN 100088:2014: Steel and steel alloys
DIN EN ISO 14025:2011-10, Environmental labels and
declarations - Type III environmental declarations - Principles EN 179
and procedures EN 179:2008-04: Building hardware - Emergency exit devices
operated by a lever handle or push pad, for use on escape
ECHA routes - Requirements and test methods
European Chemicals Agency: https://echa.europa.eu/de/home
REACH EN 1125
Registration, Evaluation, Authorisation and Restriction of EN 1125:2008-04: Building hardware - Panic exit devices
Chemicals (REACH), Regulation (EC) No 1907/2006 operated by a horizontal bar, for use on rescue routes -
Requirements and test methods
GaBi
Sphera Solutions GmbH Gabi Software System and Database EN 1634
for Life Cycle Engineering 1992-2020 Version 10.0.0.71 EN 1634-1:2018-04: Fire resistance and smoke control tests for
University of Stuttgart Leinfelden-Echterdingen door and shutter assemblies, openable windows and elements
of building hardware - Part 1: Fire-resistance test for door and
GaBi ts documentation shutter assemblies and openable windows
GaBi life cycle inventory data documentation https://www.gabi-
software.com/support/gabi/gabidatabase2020-lci- EN 1906
documentation/ EN 1906:2012-12: Building hardware - Lever handles and knob
furniture - Requirements and test
LCA-tool dormakaba methods
LCA tool IBU-DOR-202104-LT1-EN, version 1.0, 2021
Developed by Sphera Solutions GmbH EN 13126-3
EN 13126-3:2023-04: Building hardware - Hardware for
IBU 2021 windows and door height windows -
General Instructions for the EPD programme of Institut Bauen Requirements and test methods - Part 3: Handles, primarily for
und Umwelt e.V. Version 2.0, Berlin: Institut Bauen und Umwelt tilt and turn, Tilt-first and turn-only hardware
e.V., 2021. www.ibu-epd.com
DIN 18082
PCR Part A DIN 18082-1:T1EErl MV:1993-02-03: Fire-resistant single-leaf
PCR – Part A: Calculation Rules for the Life Cycle Assessment steel doors (T 30-1 doors) – Dimensions and requirements
and Requirements on the Project Report according to
EN15804+A2:2019, Version 1.0, 2020, Institut Bauen und DIN 18095, Parts 1 + 2
Umwelt e.V., www.ibu-epd.com DIN 18095-1:1988-10: Smoke control doors; Concepts and
PCR Part B requirements
5 Environmental Product Declaration - OGRO - Aluminium lever and window handle CORE/PREMIUM
DIN 18095-2:1991-03: Smoke control doors; Type testing for
durability and leakage DIN 18273
DIN 18273:2015-07: Building hardware - Lever handle units for
DIN 18255 fire doors and smoke control doors - Terms and definitions,
DIN 18255:2020-05: Building hardware - Door lever handles, dimensions, requirements, testing and marking
backplates and escutcheons - Definitions, dimensions,
requirements and marking DIN 4102
DIN 4102-1:1998-05 Fire behaviour of building materials and
DIN 18257 building components – Part 1: Building materials, concepts,
DIN 18257:2022-02: Building hardware - Security plates - requirements and tests
Definitions, measurements, requirements, marking
6 Environmental Product Declaration - OGRO - Aluminium lever and window handle CORE/PREMIUM
Publisher
Institut Bauen und Umwelt e.V. +49 (0)30 3087748- 0
Hegelplatz 1 info@ibu-epd.com
10117 Berlin www.ibu-epd.com
Germany
Programme holder
Institut Bauen und Umwelt e.V. +49 (0)30 3087748- 0
Hegelplatz 1 info@ibu-epd.com
10117 Berlin www.ibu-epd.com
Germany
Author of the Life Cycle Assessment
dormakaba International Holding GmbH +49 2333 793-0
DORMA Platz 1 info.de@dormakaba.com
58256 Ennepetal www.dormakaba.com
Germany
Owner of the Declaration
OGRO Beschlagtechnik GmbH +49 (0)2053 495-0
Donnenberger Straße 2 info@ogro.de
42553 Velbert www.ogro.de
Germany
7 Environmental Product Declaration - OGRO - Aluminium lever and window handle CORE/PREMIUM
