ENVIRONMENTAL PRODUCT DECLARATION
as per ISO 14025 and EN 15804+A2
Owner of the Declaration VELUX Group
Publisher Institut Bauen und Umwelt e.V. (IBU)
Programme holder Institut Bauen und Umwelt e.V. (IBU)
Declaration number EPD-VEL-20220114-CBB3-EN
Issue date 24/05/2022
Valid to 23/05/2027
VELUX flashings for flat roofing material
VELUX Group
www.ibu-epd.com | https://epd-online.com
General Information
VELUX Group VELUX flashings for flat roofing material
Programme holder Owner of the declaration
IBU – Institut Bauen und Umwelt e.V. VELUX Group
Hegelplatz 1 Ådalsvej 99
10117 Berlin 2970 Hørsholm
Germany Denmark
Declaration number Declared product / declared unit
EPD-VEL-20220114-CBB3-EN 1m² flashing for flat roofing material EDN
The declared unit is based on the configuration of a standard size window
measuring 0.78m x 1.178m.
This declaration is based on the product category rules: Scope:
Windows and doors , 01/08/2021 Productline EDN - Flashing; manufactured by VELUX in France, Hungary,
(PCR checked and approved by the SVR) Poland, Denmark and China for sale in Europe.
Declaration according to ISO 14025 and EN 15804 describing specific
Issue date environmental performances of the construction product.
The owner of the declaration shall be liable for the underlying information
24/05/2022
and evidence; the IBU shall not be liable with respect to manufacturer
information, life cycle assessment data and evidences.
Valid to
The EPD was created according to the specifications of EN 15804+A2. In
23/05/2027 the following, the standard will be simplified as EN 15804.
Verification
The standard EN 15804 serves as the core PCR
Independent verification of the declaration and data according to ISO
14025:2011
internally X externally
Dipl.-Ing. Hans Peters
(Chairman of Institut Bauen und Umwelt e.V.)
Florian Pronold Prof. Dr. Birgit Grahl,
(Managing Director Institut Bauen und Umwelt e.V.) (Independent verifier)
1 Environmental Product Declaration - VELUX Group - VELUX flashings for flat roofing material
Product
Name Value Unit
Product description/Product definition
Aluminium 96 %
The VELUX flashings for flat roofing material are products for
sale in the European market. This group of flashings cover a Galvanized steel 1 %
large range of different flashing types for profiled roofing Stainless steel 0.4 %
material. Polybutadiene 1 %
Polyethylene LD 1 %
The different flashing types fit for installation with either a single
window configuration or configurations of multiple windows REACH
installed adjacent to each other. All the flashings consist mainly
of aluminium. This product/article/at least one partial article contains
substances listed in the candidate list (date: 17.01.2022)
The calculations are based on the representative flashing for exceeding 0.1 percentage by mass: no.
flat roofing material named EDN. In the LCA, the EDN was
assessed to be a conservative choice for a representative Recycled content
flashing for profiled roofing material type. For the use and
application of the product the respective national provisions at
the place of use apply, in Germany for example the building
codes of the federal states and the corresponding national
specifications.
Application The values stated in the table relate to the recycled material
VELUX flashings for flat roofing material are used in renovation streams in VELUX production.
and new build. Either installed as a single window or in a
combination of multiple windows.
Reference service life
Technical Data A calculation of the reference service life according to ISO
15686 is not possible.
Constructional data
The Bundesinstitut für Bau, Stadt und Raumforschung/Federal
Name Value Unit
office for building and regional planning (BBSR)
Reaction to fire EN 13501-1 E class table declares for the complete roof window a service life
Performance data of the product with respect to its dependent on the applied window frame material between 25
characteristics in accordance with the relevant technical and ≥ 50 years. This includes collars and flashings as declared
provision (no CE-marking). with this EPD.
Base materials/Ancillary materials
LCA: Calculation rules
Declared Unit C1: a manual demolition is assumed, resulting in indicator value
The declared unit is one m² related to a reference window, that "0".
the flashing is installed in connection with. C2: For the transport to EoL by truck a distance of 50 km is
assumed.
The declared unit is based on the representative product C3: A scenario for the incineration of plastics in a waste
measuring 0.78m x 1.178m. incineration plant (WIP) is assumed.
Declared unit
The EoL-Scenario does not assume waste to be disposed of on
Name Value Unit
a landfill site. Module C4 is declared as "0".
Declared unit 1 m2
Weight per area 3.30 kg/representative product Benefits for the next product system D:
Weight per area 3.59 kg/declared unit Resulting electrical and thermal energy from the WIP, avoiding
the generation of electricity and heat via fossil fuels, is
considered.
The amount of metals after the reduction due to the net-flow
System boundary
calculations is sent to a recycling process. The effort for
Type of EPD: Cradle to gate - with options. The following life
recycling, as well as the benefit for the regained metals are
cycle stages were considered:
declared in module D.
Production stage A1-A3:
Contribution of waste flows is considered in the modules where
Consideration of the production of raw materials and their
they occur.
processing; transport of major material to the manufacturing
site; assembly of semi-finished products to the final product; Geographic Representativeness
packaging material (including waste paper input for paper and
Land or region, in which the declared product system is
cardboard).
manufactured, used or handled at the end of the product´s
lifespan: Europe
End-of-Life stage C1, C2, C3:
2 Environmental Product Declaration - VELUX Group - VELUX flashings for flat roofing material
the product-specific characteristics of performance, are taken
Comparability into account. The software GaBi is used accompanied by the
Basically, a comparison or an evaluation of EPD data is only GaBi background data base (version 2021.2, 2021).
possible if all the data sets to be compared were created
according to EN 15804 and the building context, respectively
LCA: Scenarios and additional technical information
Characteristic product properties of biogenic carbon
The following declared values refer to the declared unit of 1m².
Information on describing the biogenic Carbon Content at
factory gate Reference service life
The declared biogenic content comprises the paper manual Name Value Unit
and the packaging material consisting of cardboard, paper and
Life Span (according to BBSR) depending on 25 -
wood. As module A5 is not declared, the information on a
window frame material 50
packaging supports further EoL calculations.
Name ValueUnit End of life (C1-C4)
kg Name Value Unit
Biogenic carbon content in product -
C Collected separately waste type waste type 3.59 kg
Biogenic carbon content in accompanying 0.735 kg Recycling 3.5 kg
packaging C
Energy recovery 0.07 kg
The value refers to the following packaging material (per 1m²):
Paper (manual): 0.020kg, Cardboard packaging: 1.684kg, Reuse, recovery and/or recycling potentials (D), relevant
Paper insert: 0.007kg, PE-LD: 0.013kg scenario information
Name Value Unit
Note: 1 kg of biogenic carbon is equivalent to 44/12 kg of CO .
2 Aluminium (net-flow calculation) 2.31 kg/1m² product
Steel (net-flow calculation) 0.04 kg/1m² product
Stainless steel (net-flow calculation) 8.18E-03 kg/1m² product
3 Environmental Product Declaration - VELUX Group - VELUX flashings for flat roofing material
LCA: Results
DESCRIPTION OF THE SYSTEM BOUNDARY (X = INCLUDED IN LCA; MND = MODULE OR INDICATOR NOT DECLARED; MNR
= MODULE NOT RELEVANT)
Benefits and
Construction loads beyond
Product stage Use stage End of life stage
process stage the system
boundaries
la ire ta m w a Ry lp p u s tro p s n a rT g n iru tc a fu n a M e h t m o rf tro p s n a rTe tis e h t o t e ta g y lb m e s s A e s U e c n a n e tn ia M ria p e R tn e m e c a lp e R tn e m h s ib ru fe R y g re n e la n o ita re p Oe s u re ta w la n o ita re p Oe s u n o itc u rts n o c -e Dn o itilo m e d tro p s n a rT g n is s e c o rp e ts a W la s o p s iD -e s u e R-y re v o c e R-g n ilc y c e Rla itn e to p
A1 A2 A3 A4 A5 B1 B2 B3 B4 B5 B6 B7 C1 C2 C3 C4 D
X X X MND MND MND MND MNR MNR MNR MND MND X X X X X
RESULTS OF THE LCA - ENVIRONMENTAL IMPACT according to EN 15804+A2: 1 m² EDN
Parameter Unit A1-A3 C1 C2 C3 C4 D
Global Warming Potential total (GWP-total) kg CO 2 eq 2.3E+01 0 1.09E-02 7.29E-01 0 -1.72E+01
Global Warming Potential fossil fuels (GWP-fossil) kg CO 2 eq 2.57E+01 0 1.08E-02 7.29E-01 0 -1.72E+01
Global Warming Potential biogenic (GWP-biogenic) kg CO 2 eq -2.69E+00 0 -1.29E-05 4.45E-05 0 -4.32E-02
Global Warming Potential luluc (GWP-luluc) kg CO 2 eq 1.75E-02 0 8.85E-05 2.6E-05 0 -6.23E-03
Depletion potential of the stratospheric ozone layer (ODP) kg CFC11 eq 2.7E-11 0 2.14E-18 2.11E-16 0 -1.9E-14
Acidification potential of land and water (AP) mol H+ eq 1.14E-01 0 2.14E-05 9.15E-05 0 -8.64E-02
Eutrophication potential aquatic freshwater (EP-freshwater) kg P eq 7.7E-05 0 3.22E-08 3.26E-08 0 -6.85E-06
Eutrophication potential aquatic marine (EP-marine) kg N eq 1.86E-02 0 8.86E-06 2.46E-05 0 -1.1E-02
Eutrophication potential terrestrial (EP-terrestrial) mol N eq 1.98E-01 0 1E-04 4.17E-04 0 -1.2E-01
Formation potential of tropospheric ozone photochemical oxidants kg NMVOC
5.5E-02 0 1.91E-05 7.12E-05 0 -3.42E-02
(POCP) eq
Abiotic depletion potential for non fossil resources (ADPE) kg Sb eq 5.94E-06 0 9.6E-10 3.07E-09 0 -1.88E-06
Abiotic depletion potential for fossil resources (ADPF) MJ 3.56E+02 0 1.44E-01 2.7E-01 0 -2.19E+02
m3 world eq
Water use (WDP) 3.6E+00 0 1.01E-04 7.49E-02 0 -2.82E+00
deprived
RESULTS OF THE LCA - INDICATORS TO DESCRIBE RESOURCE USE according to EN 15804+A2: 1 m² EDN
Parameter Unit A1-A3 C1 C2 C3 C4 D
Renewable primary energy as energy carrier (PERE) MJ 1.27E+02 0 8.3E-03 5.84E-02 0 -1.01E+02
Renewable primary energy resources as material utilization
MJ 2.73E+01 0 0 0 0 0
(PERM)
Total use of renewable primary energy resources (PERT) MJ 1.55E+02 0 8.3E-03 5.84E-02 0 -1.01E+02
Non renewable primary energy as energy carrier (PENRE) MJ 3.53E+02 0 1.45E-01 3.83E+00 0 -2.2E+02
Non renewable primary energy as material utilization (PENRM) MJ 3.56E+00 0 0 -3.56E+00 0 0
Total use of non renewable primary energy resources (PENRT) MJ 3.57E+02 0 1.45E-01 2.7E-01 0 -2.2E+02
Use of secondary material (SM) kg 2.88E+00 0 0 0 0 2.22E+00
Use of renewable secondary fuels (RSF) MJ 0 0 0 0 0 0
Use of non renewable secondary fuels (NRSF) MJ 0 0 0 0 0 0
Use of net fresh water (FW) m3 3.31E-01 0 9.51E-06 1.78E-03 0 -2.61E-01
RESULTS OF THE LCA – WASTE CATEGORIES AND OUTPUT FLOWS according to EN 15804+A2:
1 m² EDN
Parameter Unit A1-A3 C1 C2 C3 C4 D
Hazardous waste disposed (HWD) kg 6.03E-07 0 7.63E-12 4.83E-11 0 -4.88E-06
Non hazardous waste disposed (NHWD) kg 5.97E+00 0 2.27E-05 6.54E-02 0 -5.14E+00
Radioactive waste disposed (RWD) kg 2.37E-02 0 2.63E-07 1.06E-05 0 -1.32E-02
Components for re-use (CRU) kg 0 0 0 0 0 0
Materials for recycling (MFR) kg 0 0 0 3.3E+00 0 0
Materials for energy recovery (MER) kg 0 0 0 0 0 0
Exported electrical energy (EEE) MJ 0 0 0 1.6E+00 0 0
Exported thermal energy (EET) MJ 0 0 0 2.88E+00 0 0
RESULTS OF THE LCA – additional impact categories according to EN 15804+A2-optional:
1 m² EDN
Parameter Unit A1-A3 C1 C2 C3 C4 D
Disease
Incidence of disease due to PM emissions (PM) 1.2E-06 0 1.3E-10 1.25E-09 0 -9.09E-07
incidence
Human exposure efficiency relative to U235 (IR) kBq U235 eq 4.59E+00 0 3.84E-05 1.4E-03 0 -2.76E+00
Comparative toxic unit for ecosystems (ETP-fw) CTUe 1.25E+02 0 1.07E-01 1.91E-01 0 -7.94E+01
Comparative toxic unit for humans (carcinogenic) (HTP-c) CTUh 4.06E-08 0 2.17E-12 1.06E-11 0 -1.08E-08
4 Environmental Product Declaration - VELUX Group - VELUX flashings for flat roofing material
Comparative toxic unit for humans (noncarcinogenic) (HTP-nc) CTUh 2.99E-07 0 1.18E-10 1.11E-09 0 -2.12E-07
Soil quality index (SQP) SQP 1.74E+02 0 4.96E-02 6.59E-02 0 -7.21E+00
Disclaimer 1 – for the indicator 'Potential Human exposure efficiency relative to U235'.
This impact category deals mainly with the eventual impact of low dose ionizing radiation on human health of the nuclear fuel cycle. It
does not consider effects due to possible nuclear accidents, occupational exposure or radioactive waste disposal in underground
facilities. Potential ionizing radiation from the soil, radon and from some construction materials is also not measured by this indicator.
Disclaimer 2 – for the indicators 'abiotic depletion potential for non-fossil resources', 'abiotic depletion potential for fossil resources',
'water (user) deprivation potential, deprivation-weighted water consumption', 'potential comparative toxic unit for ecosystems', 'potential
comparative toxic unit for humans – cancerogenic', 'Potential comparative toxic unit for humans - not cancerogenic', 'potential soil
quality index'. The results of this environmental impact indicator shall be used with care as the uncertainties on these results are high
or as there is limited experience with the indicator.
Disclaimer 3 – for 'potential soil quality index'. Due to a data lack in the foreground data of VELUX, the result has a very high
uncertainty and refers only to the background data, which contain respective information.
References
BBSR EN ISO 14025:2011, Environmental labels and declarations —
BBSR, 24.02.2017, Nutzungsdauer von Bauteilen nach BNB Type III environmental declarations — Principles and
procedures.
DIN EN 13501
DIN EN 13501-1:2019-05: Fire classification of construction ISO 15686
products and building elements - Part 1: Classification using ISO 15686:2011-05: Buildings and constructed assets - Service
data from reaction to fire tests life planning - Part 1: General principles and framework
DIN EN ISO 10077 PCR part A
DIN EN ISO 10077-1:2020-10: Thermal performance of Calculation Rules for the Life Cycle Assessment and
windows, doors and shutters - Calculation of thermal Requirements on the Project Report according to EN
transmittance 15804+A2:2019, version 1.2, Berlin: Institut Bauen und Umwelt
e.V., 2021
EN 15804
EN 15804:2012+A2:2019, Sustainability of construction works PCR part B
— Environmental Product Declarations — Core rules for the Requirements on the EPDS for Windows and doors, version
product category of construction products. 01-2021, Berlin: Institut Bauen und Umwelt e.V.
GaBi REACH
GaBi Software and GaBi Database by Sphera Solution GmbH, Regulation (EC) No 1907/2006 of the European Parliament and
version: 2021.2, 2021 of the Council on the Registration, Evaluation, Authorisation
and Restriction of Chemicals (REACH)
IBU 2021
Institut Bauen und Umwelt e.V.: General Instructions for the Regulation (EU) No. 305/2011 (CPR)
EPD programme of Institut Bauen und Umwelt e.V., Version Regulation (EU) No 305/2011 of the European Parliament and
2.0, Berlin: Institut Bauen und Umwelt e.V., 2021, www.ibu- of the Council of 9 March 2011 laying down harmonized
epd.com conditions for the marketing of construction products and
repealingCounsicl Directive 89/106/EEC
ISO 14025
5 Environmental Product Declaration - VELUX Group - VELUX flashings for flat roofing material
Publisher
Institut Bauen und Umwelt e.V. +49 (0)30 3087748- 0
Hegelplatz 1 info@ibu-epd.com
10117 Berlin www.ibu-epd.com
Germany
Programme holder
Institut Bauen und Umwelt e.V. +49 (0)30 3087748- 0
Hegelplatz 1 info@ibu-epd.com
10117 Berlin www.ibu-epd.com
Germany
Author of the Life Cycle Assessment
Angela Schindler Umweltberatung 07553 919 9456
Tüfinger Str. 12 angela@schindler-umwelt.de
88682 Salem www.schindler-umwelt.de
Germany
Daxner & Merl GmbH +43 676 849477826
Lindengasse 39/8 office@daxner-merl.com
1070 Wien www.daxner-merl.com
Austria
Owner of the Declaration
VELUX Group +4545164726
Ådalsvej 99 jakob.roerbech@velux.com
2970 Hørsholm www.velux.com
Denmark
6 Environmental Product Declaration - VELUX Group - VELUX flashings for flat roofing material
