ENVIRONMENTAL PRODUCT DECLARATION
as per ISO 14025 and EN 15804+A2
Owner of the Declaration Fletco Carpets A/S
Programme holder Institut Bauen und Umwelt e.V. (IBU)
Publisher Institut Bauen und Umwelt e.V. (IBU)
Declaration number EPD-FLE-20220317-CBC1-EN
Issue date 17.01.2023
Valid to 16.01.2028
Woven broadloom carpet
pile material polyamide 6.6, aqueous dyeing method,
maximum total pile weight 800 g/m2
Fletco Carpets A/S
www.ibu-epd.com | https://epd-online.com
Umwelt Produktdeklaration Name des Herstellers – Name des Produkts
General Information
Fletco Carpets A/S Woven broadloom carpet
pile material PA 6.6, aqueous dyeing
method, max. total pile weight 800
g/m2
Programme holder Owner of the declaration
IBU – Institut Bauen und Umwelt e.V. Fletco Carpets A/S
Hegelplatz 1 Mads Clausens Vej 2
10117 Berlin 7441 Bording
Germany Denmark
Declaration number Declared product / declared unit
EPD-FLE-20220317-CBC1-EN 1 m2 woven broadloom carpet having a pile material of
polyamide 6.6
This declaration is based on the product Scope:
category rules: The manufacturer declaration applies to a group of
Floor coverings, 02/2018 products with a maximum total pile weight of 800 g/m2.
(PCR checked and approved by the SVR) LCA results for products of the same construction but
with a maximum total pile weight of 400 g/m2 can be
taken from the corresponding tables of the annexe.
Issue date
Specific data for every product within the declared
17.01.2023
group of products in relation to its total pile weight can
be calculated by using equation 1 given in the annexe
Valid to (see annexe chapter: 'General Information on the
16.01.2028 annexe').
The carpet is woven in the Fletco manufacturing site
Bording, Denmark and it is dyed, precoated and back
coated in the Foamtex site, Bording, Denmark.
The declaration is only valid in conjunction with a valid
GUT-PRODIS license of the product.
The owner of the declaration shall be liable for the
underlying information and evidence; the IBU shall not
be liable with respect to manufacturer information, life
cycle assessment data and evidences.
The EPD was created according to the specifications
of EN 15804+A2. In the following, the standard will be
simplified as EN 15804.
Verification
The standard EN 15804 serves as the core PCR
Independent verification of the declaration and data
according to ISO 14025:2011
Dipl. Ing. Hans Peters internally x externally
(chairman of Institut Bauen und Umwelt e.V.)
Dr. Alexander Röder Angela Schindler
(Managing Director Institut Bauen und Umwelt e.V.)) (Independent verifier)
Product
Product description/Product definition the corresponding tables of the annexe. Results for
Woven broadloom carpet having a pile material of products of the same construction but with any other
polyamide 6.6 and a woven textile backing made of total pile weight can be calculated by using equation 1
polyester with recycled content. given in the annex (see annex chapter: 'General
The carpet is colored by a continuous dyeing method. Information on the annex')
The declaration applies to a group of products with a For the placing on the market of the specific product in
maximum total pile weight of 800 g/m2. the European Union/European Free Trade Association
The LCA results are calculated for products with the (EU/EFTA) (with the exception of Switzerland)
maximum total pile weight. LCA results for products Regulation (EU) No. 305/2011 Construction Product
with a total pile weight of 400 g/m2 can be taken from
2 Environmental Product Declaration Fletco Carpets A/S – Woven broadloom carpet, total pile material max. 800 g/m² PA
6.6, aqueous dyeing method
Regulation (CPR) applies. The product needs a PRODIS using the PRODIS registration number of the
Declaration of Performance (DoP) taking into product (www.pro-dis.info) or on the manufacturer's
consideration EN 14041:2018-05, Resilient, textile and technical information section.
laminate floor coverings - Essential characteristics, and
the CE-marking. The DoP of the product can be found Base materials/Ancillary materials
on the manufacturer's technical information section.
For the application and use of the product the Name Value Unit
respective national provisions apply. Polyamide 6.6 32.5 %
Polyester 16.6 %
Application Polypropylene 1.1 %
According to the use class as defined in /EN 1307/ the Polymer dispersion (solid content) 17.5 %
products can be used in all professional area with Mineral filler 22.6 %
heavy use which require class 33 or less. Aluminum hydroxide 8.6 %
Additives 1.1 %
The specific product coverd by the EPD contains
substances listed in the ECHA candidate list
(08.07.2021) or other carcinogenic, mutagenic or
Technical Data reprotoxic (CMR) substances in categories 1A or 1B
which are not on the candidate list exceeding 0.1
percentage by mass: no
Constructional data according to EN 1307 The products are registered in the GUT-PRODIS
Name Value Unit Information System. The PRODIS system ensures the
Broadloom carpet compliance with limitations of various chemicals and
Product Form -
on rolls of 4 m width Volatile Organic Compound (VOC)-emissions and a
Type of manufacture Woven carpet - ban on the use of all substances that are listed as
Continuous dyeing 'Substances of Very High Concern' (SVHC) under
Dyeing method -
method REACH.
Yarn type Polyamide 6.6 -
Woven textile backing Reference service life
Secondary backing made of polyester with - The service life of textile floor coverings strongly
recycled content depends on the correct installation taking into account
Total pile weight max. 800 g/m² the declared use classification and the adherence to
cleaning and maintenance instructions.
Total carpet weight max. 2460 g/m2
A calculation of the reference service life according to
ISO 15686 is not possible.
Alternatively, a reference service life of 10 years can
Performance data of the product in accordance with
be assumed, during which the functional and visual
the declaration of performance with respect to its
quality is guaranteed (BNB, Nutzungsdauer von
essential characteristics according to EN 14041: 2018-
Bauteilen). The technical service life can be
05, Resilient, textile and laminate floor coverings -
significantly longer.
Essential characteristics.
Additional product properties in accordance with EN
1307 can be found on the Product Information System
LCA: Calculation rules
Declared Unit
System boundaries of modules A, B, C, D:
Modules C3, C4 and D are indicated separately for
Name Value Unit three end-of-life scenarios:
Declared unit 1 m2
Grammage 2.46 kg/m2 1 - landfill disposal
The declared unit refers to 1 m2 produced textile floor 2 - municipal waste incineration
covering. The Output of module A5 'Assembly' is 1 m2 3 - recovery in a cement plant
installed textile floor covering.
The layer thickness of the specific product covered by
the EPD can be found on the Product Information A1-A3 Production:
System PRODIS using the PRODIS registration Energy supply and production of the basic material,
number of the product (www.pro-dis.info) or on the processing of secondary material, auxiliary material,
manufacturer's technical information section. transport of the material to the manufacturing site,
emissions, waste water treatment, packaging material
and waste processing up to the landfill disposal of
residual waste (except radioactive waste). Benefits for
System boundary generated electricity and steam due to the incineration
of production waste are aggregated.
Type of EPD:
Cradle-to-gate with options, module C1-C4, module D, A4 Transport:
and additional modules A4, A5, B1, B2. Transport of the packed textile floor covering from
factory gate to the place of installation.
3 Environmental Product Declaration Fletco Carpets A/S – Woven broadloom carpet, total pile material max. 800 g/m² PA
6.6, aqueous dyeing method
C2 Transport:
A5 Installation: Transport of the carpet waste to a landfill, to the
Installation of the textile floor covering, processing of municipal waste incineration plant (MWI) or to the
installation waste and packaging waste up to the waste collection facility for recycling.
landfill disposal of residual waste (except radioactive
waste), the production of the amount of carpet that C3 Waste processing:
occurs as installation waste including its transport to C3-1: Landfill disposal needs no waste processing.
the place of installation. C3-2: Impact from waste incineration (plant with
Generated electricity and steam due to the incineration R1>0.6), generated electricity and steam are listed in
of waste are listed in the result table as exported the result table as exported energy.
energy. C3-3: Collection of the carpet waste for recovery in the
Preparation of the floor and auxiliary materials cement industry, waste processing (granulating),
(adhesives, fixing agents, PET connectors) are beyond transport to the cement plant, emissions from the
the system boundaries and not taken into account. incineration.
B1 Use: C4 Disposal:
Indoor emissions during the use stage. After the first C4-1: Impact from landfill disposal,
year, no product-related Volatile Organic Compound C4-2: The carpet waste leaves the system in
(VOC) emissions are relevant due to known VOC module C3-2,
decay curves of the product. C4-3: The pre-processed carpet waste leaves the
system in module C3-3.
B2 Maintenance:
Cleaning of the textile floor covering for a period of 1 D Recycling potential:
year: Calculated benefits result from materials exclusive
Vacuum cleaning – electricity supply secondary materials (net materials).
Wet cleaning – electricity, water consumption, D-A5: Benefits for generated energy due to
production of the cleaning agent, waste water incineration of packaging and installation waste
treatment. (incineration plant with R1 > 0.6),
The declared values in this module have to be D-1: Benefits for generated energy due to landfill
multiplied by the assumed service life of the floor disposal of carpet waste at the end of life,
covering in the building in question. D-2: Benefits for generated energy due to incineration
of carpet waste at the end-of-life (incineration plant
B3 - B5: with R1 > 0.6),
The modules are not relevant within the assumed D-3: Benefits for saved fossil energy and saved
reference service life of 10 years. inorganic material due to recovery of the carpet in a
cement plant.
B6 - B7:
No energy and water input are required for the Comparability
operation of the carpet in the use stage. The modules Basically, a comparison or an evaluation of EPD data
are not relevant and not declared. is only possible if all the data sets to be compared
were created according to EN 15804 and the building
C1 De-construction: context, respectively the product-specific
The floor covering is de-constructed manually and no characteristics of performance, are taken into account.
additional environmental impact is caused.
Background data are taken from the GaBi database,
2022-2. Remaining data gaps are covered by the
ecoinvent 3.7 database, 2020.
LCA: Scenarios and additional technical information
Characteristic product properties incineration plant.
Information on biogenic carbon Preparation of the floor and auxiliaries (adhesives,
Biogenic carbon is neither contained in the product nor fixing agents, PET connectors etc.) are not taken into
in the packaging material. account.
Maintenance (B2)
The values for cleaning refer to 1 m2 floor covering per
year.
Transport to the construction site (A4) Depending on the application based on ISO 10874, the
Name Value Unit technical service life recommended by the
Litres of fuel (truck, EURO 0-6 mix) 0.0058 l/100km manufacturer and the anticipated strain on the floor by
Transport distance 700 km customers, the case-specific useful life can be
Capacity utilisation (including empty established. Based on this useful life the effects of
55 %
runs) module B2 need to be calculated in order to obtain the
overall environmental impacts.
Installation in the building (A5)
Name Value Unit
Material loss 0.221 kg
Polyethylene packaging waste and installation waste
are considered to be incinerated in a municipal waste
4 Environmental Product Declaration Fletco Carpets A/S – Woven broadloom carpet, total pile material max. 800 g/m² PA
6.6, aqueous dyeing method
Name Value Unit integrated into the cement clinker and substitutes for
Numb original material input. VDZ e.V.
Maintenance cycle (vacuum cleaning) 208 er
/year
Numb
Maintenance cycle (wet cleaning) 1,5 er
/year
Water consumption (wet cleaning) 0.004 m3
Cleaning agent (wet cleaning) 0.09 kg
Electricity consumption 0.314 kWh
For further information on cleaning and maintenance
see www.fletcocarpets.com
Service life
Name Value Unit
Life Span (according to
10 a
BBSR)
Declared product Corresponds to the
properties (at the gate) and specifications of -
finishes EN 1307
An assumed quality of
Conforms to the
work, when installed in
manufacturer's -
accordance with the
instructions
manufacturer’s instructions
Usage conditions, e.g. Use in areas defined by
frequency of use, the use class according -
mechanical exposure to EN 1307
Maintenance e.g. required
According to the
frequency, type and quality
manufacturers -
and replacement of
instructions
components
End of Life (C1-C4)
Three different end-of-life scenarios are declared and
the results are indicated separately in module C.
Each scenario is calculated as a 100% scenario.
Scenario 1: 100 % landfill disposal
Scenario 2: 100 % municipal waste incineration (MWI)
with R1>0.6
Scenario 3: 100 % recovery in the cement industry
If combinations of these scenarios have to be
calculated this should be done according to the
following scheme:
EOL-impact = x % impact (Scenario 1)
+ y % impact (Scenario 2)
+ z % impact (Scenario 3)
with x % + y % + z % = 100 %
Name Value Unit
Collected as mixed construction waste
2.46 kg
(scenario 1 and 2)
Collected separately (scenario 3) 2.46 kg
Landfilling (scenario 1) 2.46 kg
Energy recovery (scenario 2) 2.46 kg
Energy recovery (scenario 3) 1.694 kg
Recycling (scenario 3) 0.766 kg
Reuse, recovery and/or recycling potentials (D),
relevant scenario information
Recovery or recycling potentials due to the three end-
of-life scenarios (module C) are indicated separately.
Recycling in the cement industry (scenario 3)
The organic material of the carpet is used as an
alternative fuel in a cement kiln. It mainly substitutes
for lignite (68.8 %), hard coal (23.6 %) and petrol coke
(7.6 %). The inorganic material is substantially
5 Environmental Product Declaration Fletco Carpets A/S – Woven broadloom carpet, total pile material max. 800 g/m² PA
6.6, aqueous dyeing method
LCA: Results
The LCA results refer to all declared products with a maximum total pile weight of 800 g/m2. LCA results for
products with a maximum total pile weight of 400 g/m2 can be taken from the corresponding tables of the annexe.
Results for specific products with any other total pile weight can be calculated by using equation 1 given in the
annexe (see annexe chapter: 'General Information on the annexe').
The declared result figures in module B2 have to be multiplied by the assumed service life (in years) of the floor
covering in the building under consideration.
Information on non-relevant modules:
Modules B3 - B7 are not relevant during the service life of the carpet.
Modules C3/1, C4/2 and C4/3 cause no additional impact (see chapter "LCA: Calculation rules" in this document).
Module C2 represents the transport for scenarios 1, 2 and 3. The values in column D result from module A5.
DESCRIPTION OF THE SYSTEM BOUNDARY (X = INCLUDED IN LCA; ND = MODULE OR INDICATOR NOT
DECLARED; MNR = MODULE NOT RELEVANT)
BENEFITS AND
CONSTRUCTI LOADS
PRODUCT STAGE ON PROCESS USE STAGE END OF LIFE STAGE BEYOND THE
STAGE SYSTEM
BOUNDARIES
6 Environmental Product Declaration Fletco Carpets A/S – Woven broadloom carpet, total pile material max. 800 g/m² PA
6.6, aqueous dyeing method
lairetam
waR
ylppus tropsnarT
gnirutcafunaM
eht
morf
tropsnarT
etis
eht
ot
etag
ylbmessA esU
ecnanetniaM
riapeR
tnemecalpeR tnemhsibrufeR
ygrene
lanoitarepO esu
retaw
lanoitarepO esu
noitcurtsnoc-eD
noitilomed tropsnarT
gnissecorp
etsaW
lasopsiD -esueR -yrevoceR -gnilcyceR laitnetop
A1 A2 A3 A4 A5 B1 B2 B3 B4 B5 B6 B7 C1 C2 C3 C4 D
X X X X X X X MNR MNR MNR ND ND X X X X X
RESULTS OF THE LCA - ENVIRONMENTAL IMPACT according to EN 15804+A2: 1 m² floor covering
Core Indicator Unit A1-A3 A4 A5 B1 B2 C1 C2 C3/2 C3/3 C4/1 D D/1 D/2 D/3
-
GWP-total [kg CO2-Eq.] 1.19E+11.48E-11.54E+00.00E+04.16E-10.00E+08.35E-33.73E+03.76E+01.73E-1-1.66E-10.00E+0 1.22E+0-3.25E-1
-
GWP-fossil [kg CO2-Eq.] 1.18E+11.46E-11.53E+00.00E+02.15E-10.00E+08.20E-33.73E+03.76E+01.73E-1-1.65E-10.00E+0 1.21E+0-3.24E-1
GWP-biogenic [kg CO2-Eq.] 7.60E-2 1.89E-3 7.06E-30.00E+04.16E-30.00E+01.06E-4 4.21E-4 7.99E-4 2.09E-8-8.41E-40.00E+0-6.17E-3-4.05E-4
GWP-luluc [kg CO2-Eq.] 2.77E-3 8.25E-4 3.35E-40.00E+01.96E-10.00E+04.64E-5 8.70E-5 2.06E-4 8.49E-5-1.81E-50.00E+0-1.33E-4-1.54E-4
3.19E- 8.86E- 2.91E- 4.99E- 3.41E- 5.27E- 2.34E- -1.11E- -8.14E- -4.95E-
ODP [kg CFC11-Eq.] 0.00E+03.42E-80.00E+0 0.00E+0
11 15 12 16 13 13 13 12 12 13
AP [mol H+-Eq.] 2.08E-2 8.81E-4 2.31E-30.00E+08.32E-40.00E+04.96E-5 3.78E-3 3.93E-3 5.17E-4-2.16E-40.00E+0-1.59E-3-1.14E-3
EP-freshwater [kg P-Eq.] 3.20E-5 4.42E-7 2.95E-60.00E+05.19E-60.00E+02.49E-8 3.55E-7 4.54E-7 3.26E-5-2.26E-70.00E+0-1.66E-6-3.57E-7
EP-marine [kg N-Eq.] 6.85E-3 4.32E-4 8.28E-40.00E+01.97E-40.00E+02.43E-5 1.87E-3 1.93E-3 1.14E-4-5.87E-50.00E+0-4.32E-4-3.57E-4
EP-terrestrial [mol N-Eq.] 7.26E-2 4.79E-3 8.92E-30.00E+02.83E-30.00E+02.69E-4 2.08E-2 2.16E-2 1.25E-3-6.29E-40.00E+0-4.63E-3-3.91E-3
POCP [kg NMVOC-Eq.]2.43E-2 8.17E-4 2.70E-3 4.18E-4 9.83E-40.00E+04.60E-5 4.78E-3 4.91E-3 3.68E-4-1.64E-40.00E+0-1.21E-3-1.08E-3
6.96E-
ADPE [kg Sb-Eq.] 1.85E-6 1.24E-8 1.69E-70.00E+02.30E-70.00E+0 1.45E-8 1.97E-8 1.21E-8-2.48E-80.00E+0-1.82E-7-3.09E-8
10
- - -
ADPF [MJ] 2.38E+21.98E+02.18E+10.00E+05.90E+00.00E+01.11E-11.79E+02.30E+02.47E+0 0.00E+0
2.80E+0 2.06E+14.25E+1
[m³ world-Eq
WDP 9.25E-1 1.32E-3 1.34E-10.00E+09.99E-20.00E+07.45E-5 4.44E-1 4.47E-1-1.85E-3-1.73E-20.00E+0-1.27E-1-4.87E-2
deprived]
GWP = Global warming potential; ODP = Depletion potential of the stratospheric ozone layer; AP = Acidification potential of land and water; EP =
Caption Eutrophication potential; POCP = Formation potential of tropospheric ozone photochemical oxidants; ADPE = Abiotic depletion potential for non-
fossil resources; ADPF = Abiotic depletion potential for fossil resources; WDP = Water (user) deprivation potential
RESULTS OF THE LCA - INDICATORS TO DESCRIBE RESOURCE USE according to EN 15804+A2: 1 m²
floor covering
Indicator Unit A1-A3 A4 A5 B1 B2 C1 C2 C3/2 C3/3 C4/1 D D/1 D/2 D/3
PERE [MJ] 3.35E+1 1.12E-1 3.06E+0 0.00E+0 3.69E+0 0.00E+0 6.33E-3 2.91E-1 4.34E-1 2.03E-1 -7.67E-1 0.00E+0 -5.62E+0-4.36E-1
PERM [MJ] 0.00E+0 0.00E+0 0.00E+0 0.00E+0 0.00E+0 0.00E+0 0.00E+0 0.00E+0 0.00E+0 0.00E+0 0.00E+0 0.00E+0 0.00E+0 0.00E+0
PERT [MJ] 3.35E+1 1.12E-1 3.06E+0 0.00E+0 3.69E+0 0.00E+0 6.33E-3 2.91E-1 4.34E-1 2.03E-1 -7.67E-1 0.00E+0 -5.62E+0-4.36E-1
PENRE [MJ] 1.90E+2 1.98E+0 2.34E+1 0.00E+0 5.90E+0 0.00E+0 1.12E-1 4.89E+1 4.94E+1 2.48E+0 -2.80E+0 0.00E+0 -2.06E+1-4.25E+1
PENRM [MJ] 4.87E+1 0.00E+0 -1.58E+0 0.00E+0 0.00E+0 0.00E+0 0.00E+0 -4.71E+1-4.71E+1 0.00E+0 0.00E+0 0.00E+0 0.00E+0 0.00E+0
PENRT [MJ] 2.39E+2 1.98E+0 2.18E+1 0.00E+0 5.90E+0 0.00E+0 1.12E-1 1.79E+0 2.30E+0 2.48E+0 -2.80E+0 0.00E+0 -2.06E+1-4.25E+1
SM [kg] 8.54E-2 0.00E+0 7.69E-3 0.00E+0 0.00E+0 0.00E+0 0.00E+0 0.00E+0 0.00E+0 0.00E+0 0.00E+0 0.00E+0 0.00E+0 4.30E-1
RSF [MJ] 0.00E+0 0.00E+0 0.00E+0 0.00E+0 0.00E+0 0.00E+0 0.00E+0 0.00E+0 0.00E+0 0.00E+0 0.00E+0 0.00E+0 0.00E+0 0.00E+0
NRSF [MJ] 0.00E+0 0.00E+0 0.00E+0 0.00E+0 0.00E+0 0.00E+0 0.00E+0 0.00E+0 0.00E+0 0.00E+0 0.00E+0 0.00E+0 0.00E+0 0.00E+0
FW [m³] 5.11E-2 1.27E-4 5.81E-3 0.00E+0 3.34E-3 0.00E+0 7.15E-6 1.05E-2 1.06E-2 2.90E-5 -7.33E-4 0.00E+0 -5.37E-3 -3.86E-3
PERE = Use of renewable primary energy excluding renewable primary energy resources used as raw materials; PERM = Use of
renewable primary energy resources used as raw materials; PERT = Total use of renewable primary energy resources; PENRE = Use of
non-renewable primary energy excluding non-renewable primary energy resources used as raw materials; PENRM = Use of non-
Caption
renewable primary energy resources used as raw materials; PENRT = Total use of non-renewable primary energy resources; SM = Use
of secondary material; RSF = Use of renewable secondary fuels; NRSF = Use of non-renewable secondary fuels; FW = Use of net fresh
water
RESULTS OF THE LCA – WASTE CATEGORIES AND OUTPUT FLOWS according to EN 15804+A2:
1 m² floor covering
Indicator Unit A1-A3 A4 A5 B1 B2 C1 C2 C3/2 C3/3 C4/1 D D/1 D/2 D/3
HWD [kg] 2.11E-8 9.49E-12 1.93E-9 0.00E+0 4.19E-5 0.00E+0 5.34E-132.70E-102.91E-103.82E-10-3.80E-100.00E+0 -2.80E-9-2.03E-10
NHWD [kg] 2.61E-1 2.84E-4 6.34E-2 0.00E+0 7.30E-3 0.00E+0 1.60E-5 4.38E-1 4.38E-1 2.45E+0 -1.41E-3 0.00E+0 -1.04E-2 -1.01E-1
RWD [kg] 5.21E-3 2.44E-6 4.76E-4 0.00E+0 3.76E-4 0.00E+0 1.37E-7 6.32E-5 1.00E-4 3.04E-5 -2.20E-4 0.00E+0 -1.61E-3 -9.19E-5
CRU [kg] 0.00E+0 0.00E+0 0.00E+0 0.00E+0 0.00E+0 0.00E+0 0.00E+0 0.00E+0 0.00E+0 0.00E+0 0.00E+0 0.00E+0 0.00E+0 0.00E+0
MFR [kg] 1.22E-2 0.00E+0 1.10E-3 0.00E+0 0.00E+0 0.00E+0 0.00E+0 0.00E+0 4.30E-1 0.00E+0 0.00E+0 0.00E+0 0.00E+0 0.00E+0
MER [kg] 0.00E+0 0.00E+0 0.00E+0 0.00E+0 0.00E+0 0.00E+0 0.00E+0 0.00E+0 0.00E+0 0.00E+0 0.00E+0 0.00E+0 0.00E+0 0.00E+0
EEE [MJ] 0.00E+0 0.00E+0 7.62E-1 0.00E+0 0.00E+0 0.00E+0 0.00E+0 5.68E+0 0.00E+0 0.00E+0 0.00E+0 0.00E+0 0.00E+0 0.00E+0
EET [MJ] 0.00E+0 0.00E+0 1.38E+0 0.00E+0 0.00E+0 0.00E+0 0.00E+0 1.04E+1 4.89E+1 0.00E+0 0.00E+0 0.00E+0 0.00E+0 0.00E+0
HWD = Hazardous waste disposed; NHWD = Non-hazardous waste disposed; RWD = Radioactive waste disposed; CRU = Components
Caption for re-use; MFR = Materials for recycling; MER = Materials for energy recovery; EEE = Exported electrical energy; EET = Exported
thermal energy
RESULTS OF THE LCA – additional impact categories according to EN 15804+A2-optional:
1 m² floor covering
Indicator Unit A1-A3 A4 A5 B1 B2 C1 C2 C3/2 C3/3 C4/1 D D/1 D/2 D/3
[Disease
PM 1.78E-7 5.09E-9 1.78E-8 0.00E+0 6.84E-8 0.00E+02.86E-10 1.37E-8 1.46E-8 4.97E-9 -1.79E-9 0.00E+0 0.00E+0 -1.98E-8
Incidence]
[kBq U235-
IRP 8.35E-1 3.58E-4 7.62E-2 0.00E+0 6.78E-2 0.00E+0 2.01E-5 9.70E-3 1.59E-2 4.49E-3 -3.72E-2 0.00E+0 0.00E+0 -1.01E-2
Eq.]
ETP-fw [CTUe] 1.12E+2 1.37E+0 1.03E+1 3.60E-3 2.69E+0 0.00E+0 7.73E-2 7.82E-1 1.08E+0 2.42E+0 -6.13E-1 0.00E+0 0.00E+0-7.47E+0
-2.82E- -8.46E-
HTP-c [CTUh] 3.74E-9 2.77E-113.44E-100.00E+06.21E-100.00E+01.56E-124.37E-115.05E-111.09E-10 0.00E+0 0.00E+0
11 11
HTP-nc [CTUh] 1.35E-7 1.65E-9 1.26E-8 2.60E-11 9.46E-9 0.00E+09.26E-11 2.77E-9 3.11E-9 9.11E-9 -1.08E-9 0.00E+0 0.00E+0 -4.95E-9
SQP [-] ND ND ND ND ND ND ND ND ND ND ND ND ND ND
PM = Potential incidence of disease due to PM emissions; IR = Potential Human exposure efficiency relative to U235; ETP-fw = Potential
Caption comparative Toxic Unit for ecosystems; HTP-c = Potential comparative Toxic Unit for humans (cancerogenic); HTP-nc = Potential
comparative Toxic Unit for humans (not cancerogenic); SQP = Potential soil quality index
The SQP indicator is not given due to considerable uncertainties in the calculation.
The result figures given in module B2 refer to a period of 1 year because a reference service life is not declared.
They have to be multiplied by the assumed service life (in years) of the floor covering in the building under
consideration.
Disclaimer 1 – for the indicator “Potential Human exposure efficiency relative to U235”.
This impact category deals mainly with the eventual impact of low dose ionizing radiation on human health of the
nuclear fuel cycle. It does not consider effects due to possible nuclear accidents, occupational exposure nor due
to radioactive waste disposal in undergroundfacilities. Potential ionizing radiation from the soil, from radon and
from some construction materials is also not measured by this indicator.
Disclaimer 2 – for the indicators “abiotic depletion potential for non-fossil resources”, “abiotic depletion potential
for fossil resources”, “water (user) deprivation potential, deprivation-weighted water consumption”, “potential
comparative toxic unit for ecosystems”, “potential comparative toxic unit for humans – cancerogenic”, “Potential
comparative toxic unit for humans - not cancerogenic”, “potential soil quality index”.
The results of this environmental impact indicator shall be used with care as the uncertainties on these results are
high or as there is limited experienced with the indicator.
References
EN 1307 EN 16810
DIN EN 1307: 2014+A1:2016+A2:2018-05: Textile DIN EN 16810: 2017-08: Resilient, textile and laminate
floor coverings - Classification floor coverings – Environmental product declarations –
Product category rules
EN 13501-1
DIN EN 13501-1:2019-05: Fire classification of ISO 10874
construction products and building elements - Part 1: DIN EN ISO 10874: 2012+A1:2021-04: Resilient,
Classification using data from reaction to fire tests textile and laminate floor coverings - Classification
EN 14041 ISO 14025
DIN EN 14041: 2018-05 and DIN EN 14041: 2008-05: DIN EN /ISO 14025:2011-10/, Environmental labels
Resilient, textile and laminate floor coverings - and declarations — Type III environmental
Essential characteristics declarations — Principles and procedures
EN 15804 ISO 14040
DIN EN 15804:2012+A2:2019 + AC:2021, DIN EN ISO 14040:2006+A1:2020 Environmental
Sustainability of construction works — Environmental management - Life cycle assessment - Principles and
Product Declarations — Core rules for the product framework
category of construction products
7 Environmental Product Declaration Fletco Carpets A/S – Woven broadloom carpet, total pile material max. 800 g/m² PA
6.6, aqueous dyeing method
ISO 14044
DIN EN ISO 14044:2006+A1:2018+A2:2020 ecoinvent
Environmental management - Life cycle assessment - ecoinvent, Zurich, Switzerland, database version 3.7,
Requirements and guidelines published September 2020
ISO 15686 GaBi database
ISO 15686: Buildings and constructed assets - GaBi Software-System and Database for Life Cycle
Service life planning Engineering, thinkstep AG, Leinfelden-Echterdingen,
ISO 15686-1: 2011-05: Part 1: General principles and 2022-2
framework
ISO 15686-2: 2012-05: Part 2: Service life prediction PCR Part A
procedures Product Category Rules for Building-Related Products
ISO 15686-7: 2017-04: Part 7: Performance and Services Part A: Calculation Rules for the Life
evaluation for feedback of service life data Cycle Assessment and Requirements on the Project
from practice Report according to EN 15804+A2:2019, V1.3, Berlin:
ISO 15686-8: 2008-06: Part 8: Reference service life Institut Bauen und Umwelt e.V. (IBU), August 2022
and service-life estimation
PCR Part B
Regulation (EU) No. 305/2011 Product Category Rules for Building-Related Products
Regulation No. 305/2011 Construction Products and Services
Regulation (CPR) of the European Council and of the Part B: Requirements on the EPD for floor coverings,
European Parliament, April 2011 V1.3, Berlin: Institut Bauen und Umwelt e.V. (IBU),
September 2022
General Instructions for the IBU-EPD Program
General Instructions for the EPD-Program of the PRODIS
Institut Bauen und Umwelt e.V., The Preparation of Product Information System (PRODIS) of the
Environmental Product Declarations - EPDs, version European Carpet Industry, Gemeinschaft
2.0, Institut Bauen und Umwelt e.V., Berlin, January umweltfreundlicher Teppichboden e.V (GUT) and
2021, www.ibu-epd.de European Carpet and Rug Association
(ECRA), http://www.pro-dis.info
BBSR
Bundesinstitut für Bau-, Stadt- und Raumforschung REACH
(BBSR) im Bundesamt für Bauwesen und Regulation (EC) No 1907/2006 of the European
Raumordnung (BBR), Bonn Parliament and of the Council of 18 December 2006
concerning the Registration, Evaluation, Authorisation
BNB, Nutzungsdauer von Bauteilen and Restriction of Chemicals (REACH), June 2017
Bewertungssystem Nachhaltiges Bauen (BNB),
Nutzungsdauer von Bauteilen, Bundesministerium des VDZ e.V.
Inneren, für Bau und Heimat, 24.02.2017 Association of German Cement Works, Ed. Environ-
mental Data of the German Cement Industry 2020
ECHA candidate list
Candidate List of substances of very high concern
(SVHCs) for authorisation, 08.07.2021, last update
26.07.2022, European Chemicals Agency (ECHA),
Helsinki, Finland
8 Environmental Product Declaration Fletco Carpets A/S – Woven broadloom carpet, total pile material max. 800 g/m² PA
6.6, aqueous dyeing method
Publisher
Institut Bauen und Umwelt e.V. Tel +49 (0)30 3087748- 0
Hegelplatz 1 Fax +49 (0)30 3087748- 29
10117 Berlin Mail info@ibu-epd.com
Germany Web www.ibu-epd.com
Programme holder
Institut Bauen und Umwelt e.V. Tel +49 (0)30 - 3087748- 0
Hegelplatz 1 Fax +49 (0)30 – 3087748 - 29
10117 Berlin Mail info@ibu-epd.com
Germany Web www.ibu-epd.com
Author of the Life Cycle
Assessment Tel +49 (0)241 96843 410
Gemeinschaft umweltfreundlicher Fax +49 (0)241 96843 400
Teppichboden (GUT) e.V. Mail mail@gut-ev.de
Schönebergstraße 2 Web www.gut-ev.org
52068 Aachen
Germany
Owner of the Declaration
Fletco Carpets A/S Tel +45 (0)96 60 30 00
Mads Clausens Vej 2 Fax +45 (0)96 60 30 60
7441 Bording Mail fletco@fletco.dk
Denmark Web www.fletcocarpets.com
