ENVIRONMENTAL PRODUCT DECLARATION
as per ISO 14025 and EN 15804+A2
Owner of the Declaration Unilin B.V. Division Panels
Publisher Institut Bauen und Umwelt e.V. (IBU)
Programme holder Institut Bauen und Umwelt e.V. (IBU)
Declaration number EPD-UNI-20230379-IBJ1-EN
Issue date 31.10.2023
Valid to 30.10.2028
Unilin Melamine Faced MDF board
Unilin B.V. Division Panels
www.ibu-epd.com | https://epd-online.com
1. General Information
Unilin B.V. Division Panels Unilin Melamine Faced MDF board
Programme holder Owner of the declaration
IBU – Institut Bauen und Umwelt e.V. Unilin B.V. Division Panels
Hegelplatz 1 Ooigemstraat 3
10117 Berlin 8710 Wielsbeke
Germany Belgium
Declaration number Declared product / declared unit
EPD-UNI-20230379-IBJ1-EN 1 m² of Unilin melamine faced MDF board (11.24 kg/m²)
This declaration is based on the product category rules: Scope:
Wood-based panels, 01.08.2021 The scope of this EPD extends to Unilin's entire melamine faced medium
(PCR checked and approved by the SVR) density fiberboard (MDF) range. The declared values refer to the sales-
weighted average product. These fiberboards are produced in the following
manufacturing sites:
Issue date
Raw board
31.10.2023
• Bazeilles, France
• Vielsalm, Belgium
Valid to
Melamine faced board
30.10.2028
• SPANO, Oostrozebeke, Belgium
• BOSPAN, Wielsbeke, Belgium
The owner of the declaration shall be liable for the underlying information
and evidence; the IBU shall not be liable with respect to manufacturer
information, life cycle assessment data and evidences.
The EPD was created according to the specifications of EN 15804+A2. In
the following, the standard will be simplified as EN 15804.
Verification
Dipl.-Ing. Hans Peters The standard EN 15804 serves as the core PCR
(Chairman of Institut Bauen und Umwelt e.V.)
Independent verification of the declaration and data according to ISO
14025:2011
internally X externally
Florian Pronold Mr Olivier Muller,
(Managing Director Institut Bauen und Umwelt e.V.) (Independent verifier)
1 Environmental Product Declaration - Unilin B.V. Division Panels - Unilin Melamine Faced MDF board
2. Product
2.1 Product description/Product definition The values for specific commercial references and thicknesses
The Unilin melamine faced MDF board consists of a raw can vary from the declared ones. Please contact Unilin's sales
fiberboard that is pressed with an impregnated paper, both on team or info.panels@unilin.com for more information.
the product's front and backside. The decor on the panel is
obtained by applying a printed decor paper on the raw board. 2.2 Application
The texture is pressed into the melamine surface under high Melamine faced fiberboards are commonly used for interior
pressure and high temperature using a special press plate furniture and decorative interior design. The panels are used in
technology. both residential and commercial projects. Target segments are
retail, office and hotel. The main applications for a melamine
The fiberboard is available with different compositions (moisture faced panel are listed below:
resistant, fire retardant, …) and in different sizes. The surface
• Furniture (e.g., bedroom cupboards, sideboards, bed
does not require further treatment and can be applied in all
frames)
types of interior projects. The melamine faced board is durable,
• General interior design (e.g. counters, shelves)
scratch resistant, colorfast and easy to maintain. More than 200
• Walls
designs are available in Unilin's Decorative range (e.g. woods,
• Worktops, tabletops, desktops
plain colors and materials).
• Product presentations, exhibition stands, displays
• Doors
For the placing on the market of the product in the European
Union/European Free Trade Association (EU/EFTA) (with the
Unilin's melamine faced fiberboards can be used in a variety of
exception of Switzerland) Regulation (EU) No. 305/2011 (CPR)
applications, classified according EN 622-5:2010:
applies. The product needs a declaration of performance
according: • MDF : General purpose boards for use in dry conditions
• MDF.H : General purpose boards for use in humid
• EN 13986:2004+A1:2015, Wood-based panels for use
conditions
in construction – Characteristics, valuation of conformity
• MDF.LA : Load-bearing boards for use in dry conditions
and marking
• MDF.HLS : Load-bearing boards for use in humid
• EN 14322:2021, Wood-based panels - Melamine faced
conditions
boards for interior uses - Definition, requirements and
• L-MDF : Light MDF boards for use in dry conditions
classification
• L-MDF.H : Light MDF boards for use in humid conditions
• EN 622-5:2010, Fibreboards - Specifications - Part 5:
• UL1-MDF : Ultra-light MDF boards for use in dry
Requirements for dry process boards (MDF)
conditions
• UL2-MDF : Ultra-light MDF boards for use in dry
For the application and use the respective national provisions
conditions
apply.
All melamine faced fiberboards demonstrate low formaldehyde
The results in this EPD refer to the environmental impact of a
emissions (since the core board is coated). For some national
melamine faced MDF board with a sales-weighted average.
regulations (like CARB2, TSCA Title VI) specific low emissions
The composition and thickness of this product was obtained by
requirements apply to the core board. These core boards are
averaging the composition of Unilin's entire melamine faced
available in the LF, LF3,LF+ & NAF ranges.
fiberboard portfolio based on the annual sales volumes. The
declared impact is thus sales-weighted representative for the
The FR (Fire Retardant) fiberboard range is suited for
following commercial references at thicknesses 8 - 40 mm:
applications where increased fire protection is required.
• Unilin Evola (Basic)/Customized Design - Fibrabel
(Black) (LF+/NAF) 2.3 Technical Data
• Unilin Evola (Basic)/Customized Design - Fibrabel FR Technical characteristics vary by product variant and thickness.
(Uncoloured) More detailed product-specific data, technical data sheets and
• Unilin Evola (Basic)/Customized Design - Fibrabel MR the CE declaration of performance are available on
(Uncoloured) (FR) (NAF/LF+) www.unilinpanels.com.
• Unilin Evola (Basic)/Customized Design - Fibralux FR Constructional and surface data
(Black/Uncoloured)
The table below summarizes the technical performance of
• Unilin Evola (Basic)/Customized Design - Fibralux MR
Unilin's melamine faced fiberboard for some parameters. The
(FR) (Black/Grey/Uncoloured) (NAF/LF+)
values below apply to the product range. Performances can
• Unilin Evola (Basic)/Customized Design - Fibralux (LF
depend on the core board type. Please check the specific
+/NAF)
"Declaration Of Performance" of the products available on
• Unilin Evola (Basic)/Customized Design - Fibralux Pro
www.unilinpanels.com. Specific properties of the declared
(P/MR) (Uncoloured) (LF+/NAF)
sales-weighted product are available in 3.10.
• Unilin Evola (Basic)/Customized Design - Fibrofit (LF/LF
+)
• Unilin Evola (Basic)/Customized Design - Fibrofit MR
(Uncoloured) (LF/LF+)
• Unilin Evola (Basic)/Customized Design - Fibromax
(LF/LF+)
• Unilin Evola (Basic)/Customized Design - Fibromax MR
(Uncoloured) (LF/LF+)
• Unilin Evola (Basic)/Customized Design - Fibromax Pro
(MR) (LF/LF+)(Uncoloured)
2 Environmental Product Declaration - Unilin B.V. Division Panels - Unilin Melamine Faced MDF board
Name Value Unit
2.5 Base materials/Ancillary materials
Grammage @ 15.9 mm
11.24 kg/m² The data below details the sales-weighted average composition
(EN 323)
of the Unilin melamine faced fiberboard. This melamine faced
Bending strength (EN
Depends on core board N/mm² board has a sales-weighted thickness of 15.9 mm.
310)
E-modulus (EN 310) Depends on core board N/mm² Compostion raw board
Thermal conductivity (EN The raw MDF board has a density of 685 kg/m³ and consists of
0.10 W/(mK)
13986) fresh wood, glue, additives and moisture. The glue is either
Water vapour µ based on a (melamine) urea formaldehyde (M(UF)) mixture or
permeability (EN 13986) 26 wet/dry pMDI (polymeric form of 4,4'-Methylene diphenyl diisocyanate).
The additives added depend heavily on the specific commercial
Sound absorption 250
0.10 reference (e.g. wax emulsion, fire retardant based on inorganic
500 HZ (EN 13986)
salts).
Sound absorption 1000
0.20 Name Value Unit
2000 HZ (EN 13986)
Fresh wood 82 %
E1(*); E0.5 (**);
Formaldehyde CARB/TSCA Title VI (***); Glue 11 %
F**** (****) Additives 1 %
Surface Soundness (EN Moisture 6 %
> 1 N/mm²
311)
The fresh wood is 100 % recovered wood, predominantly
Thickness tolerance (EN
+/- 0.2 mm sourced from sustainable forest management activities and
324)
sawmills (residues & co-products), and mainly consists of
spruce, beech and birch.
Different formaldehyde emission standards are available
(*) E1 - According to EN 13986+A1:2015 : Composition melamine faced board (15.9 mm)
The sales-weighted average product has a grammage of 11.24
• a limit value of 0.1 ppm may not be exceeded by EN
kg/m² and consists of a raw MDF board and 2 impregnated
717-1 emission chamber method OR
decor paper layers, covering the front and back of the core
• a limit value of 8 mg HCHO/100 g according to ISO
board. The decor papers are impregnated with an
12460-5
urea/melamine formaldehyde resin to ensure adhesion to the
surface of the raw board. This impregnated decor paper has a
(**) E0.5 - According to the ChemVerbotsV :
sales-weighted average grammage of 173 g/m².
• a limit value of 0.1 ppm according to EN 16516 OR
• a limit value of 0.05 ppm according to EN 717-1 The melamine faced MDF board thus has the following
composition:
(***) CARB 2/TSCA Title VI - According to California Air
• Raw board: 97 %
Resources Board & the US Toxic Substances Control Act
• Impregnated decor paper (front + back): 3 %
(TSCA Title VI) :
• a limit value of 0.09 ppm according to ASTM E1333 or The composition of specific commercial references and
ASTM D6007 thicknesses can differ from the values depicted above and can
(****) F**** - According to Japanese standard JIS A 5908 be obtained by reaching out to info.panels@unilin.com.
• a limit value of 0.3 mg/L according to JIS A 1460
Unilin's melamine faced fiberboard range contains no
desiccator
Substances of Very High Concern (SVHCs) or Category 1A or
1B CMR-substances (as defined by ECHA) above 0.1 % by
Performance data are consistent with the product's declaration
weight: No
of performance with respect to its essential characteristics
The MDF boards further contain no biocides as defined under
according to:
the EU Biocidal Products Ordinance No. 528/2012 nor are the
• EN 13986:2004+A1:2015, Wood-based panels for use boards treated with such substances.
in construction – Characteristics, valuation of conformity
and marking 2.6 Manufacture
• EN 14322:2021, Wood-based panels - Melamine faced Raw board
boards for interior uses - Definition, requirements and 1. Round wood is collected to produce the fiberboards.
classification 2. The bark is removed from the round wood logs.
• EN 622-5:2010, Fibreboards - Specifications - Part 5: 3. The logs are chopped to wood chips.
Requirements for dry process boards (MDF) 4. The wood chips are defibrated under high pressure in a
refiner.
2.4 Delivery status
5. The board is produced by introducing the fibermat into a
Unilin's melamine faced MDF boards are available in a diverse
press, which compresses it under higher pressure and
range of dimensions:
temperature.
• Length: 2000 - 5600 mm 6. The board is sanded, cut into panels and finished
• Width: 1220 - 2100 mm depending on the intended application.
• Thickness: 3 - 54 mm
Melamine faced board
Please contact Unilin's sales team or info.panels@unilin.com
1. The raw decor paper is impregnated with an
for more information on available dimensions of specific
urea/melamine formaldehyde resin.
products.
3 Environmental Product Declaration - Unilin B.V. Division Panels - Unilin Melamine Faced MDF board
2. The impregnated paper is dried, cut to the correct size heavily on its chemical composition (i.e. presence of fire
and stacked on pallets or rolls. retardants). The products have the following fire behavior
3. The press plates, which contain the required surface (according to EN13501-1):
finish, are placed into the melamine press facing the
front- as well as the backside of the panel. The CE AVCP Class 4 :
impregnated paper is positioned on both sides of the
• Unilin Evola (Basic)/Customized Design -
raw board.
Standard/Moisture resistant fiberboards (excl. fire
4. The hot press closes for certain amount of time, during
retardant): D-s2,d0 (≥ 9 mm/ Bulk density > 600 kg/m³)
which the resin bonds the decor paper to the raw board.
5. The panel undergoes an additional quality check and is
CE AVCP Class 1 :
removed if necessary
6. After cooling down, the melamine faced board can be • Unilin Evola (Basic)/Customized Design – Fibralux FR :
stacked on a pallet. B-s2,d0 (10 mm)
• Unilin Evola (Basic)/Customized Design – Fibralux FR :
2.7 Environment and health during manufacturing B-s1,d0 (12-25 mm)
Unilin's plant management policy is fully integrated in the daily • Unilin Evola (Basic)/Customized Design – Fibralux FR
operation and governance of its production plants. The aim is to Black : B-s1,d0 (12-25 mm)
adhere to legal requirements, minimize negative environmental • Unilin Evola (Basic)/Customized Design – Fibralux MR
effects on its neighbors, co-workers and surroundings, and FR NAF: B-s1,d0 (12-25 mm)
constantly improve environmental performance. The Bazeilles Fire reaction classes are part of the CE Declaration of
plant is ISO 9001 and ISO 50001 certified. The Vielsalm site is Performance available on Unilin Panels' website
certified under ISO 9001, ISO 14001 and ISO 45001. The www.unilinpanels.com.
BOSPAN and SPANO plants have achieved the ISO 9001
certificate. Water
The melamine faced board does not contain substances that
The implementation of Unilin's One Home Sustainability may potentially contaminate water through leaching. However,
Strategy and its Zero Harm Safety Policy have further set clear it is important, to ensure that the product is not subjected to
targets to among others reduce the carbon footprint of its continuous exposure to moisture. Prolonged contact with water
production activities, improve the overall resource efficiency may result in the degradation of the product.
and enhance the safety and well-being at its production sites.
Mechanical destruction
2.8 Product processing/Installation When subjected to mechanical stress, the product displays a
The Unilin melamine faced MDF board can be processed (e.g. tendency towards brittleness. This could result in the formation
sawing, milling, drilling) using common utility tools and of splinters and sharp broken edges, which may pose a risk of
machinery. It is advised to wear a dust mask when tools are injury.
used without dust extraction. More specific processing and
health information is available at www.unilinpanels.com. 2.14 Re-use phase
Reuse/Recycling
2.9 Packaging When a building or furniture has reached its end-of-life phase,
Product packaging is used to protect the product from damage the Unilin melamine faced fiberboard can easily be abstracted
during transport. Wood-based chipboards, cardboard, stretch and collected if selective dismantling/sorting takes place. After
foil and PET packaging straps are used as packaging materials. collection, the end-of-life fiberboard can be reused for the same
(or different) purpose if possible.
2.10 Condition of use
The product's composition remains unchanged during its use Energy Recovery
and is therefore the same as stated in section 2.5. The glue, In line with the cascading use of wood-based products, the
resin and additives are permanently bonded to the wood and reuse of the end-of-life MDF should be prioritized. However, if
paper through an irreversible curing process. this is not feasible, the board can be used as a secondary fuel
in approved energy power plants. Its relatively high calorific
2.11 Environment and health during use
value enables power plants to effectively produce renewable
Based on current knowledge, using Unilin's melamine faced heat and electricity.
fiberboard as intended poses no risks to health, water, air or
soil. Small amounts of natural wood constituents could 2.15 Disposal
potentially be released, but aside from negligible amounts of Jobsite and post-consumer MDF-waste (e.g. from demolition
formaldehyde, no harmful emissions have been detected. projects) should be reused/recycled where possible, in line with
the cascade principle. Should this not be possible, the waste
2.12 Reference service life
must be utilized for energy recovery as opposed to being
The reference service life (RSL) of the product depends landfilled (in accordance with EWC waste codes
significantly on its field of use. Please contact Unilin's sales 170201/030105).
team or info.panels@unilin.com for more specific information
on the product's lifespan in a given set of conditions. Waste from packaging materials, which protect the product
from damage during transport, can be reused and recycled if
The RSL of a melamine faced MDF board can vary from 10 to sorted correctly.
40 years depending on its area of application; according to the
BBSR table "BNB Nutzungsdauern von Bauteilen (2017)". 2.16 Further information
Please contact Unilin's sales team or reach out to
2.13 Extraordinary effects
info.panels@unilin.com for additional information.
Fire
The fire resistance of the melamine faced fiberboard depends
4 Environmental Product Declaration - Unilin B.V. Division Panels - Unilin Melamine Faced MDF board
3. LCA: Calculation rules
exported from the system in C3.
3.1 Declared Unit
The declared information and values refer to 1 m² of Unilin C4: Waste Disposal
melamine faced fiberboard with a sales-weighted average This module describes the loads and emissions attributed to
composition, grammage of 11.24 kg/m² and thickness of 15.9 the disposal of the product after waste processing. As the end-
mm. of-life product leaves the system in C3 as a secondary fuel, no
Declared unit and mass reference environmental impact is declared in C4.
Name Value Unit
D: Loads and Benefits beyond the System Boundaries
Declared unit 1 m2 Module D describes the loads and benefits related to the use of
Grammage 11.24 kg/m2 the end-of-life MDF as a secondary fuel. This involves the
Layer thickness 0.0159 m energy recovery of post-consumer fiberboard waste, where it
replaces a European-averaged mix of electricity and heat.
This EPD reports the environmental impact of the Unilin
melamine faced MDF board. Its composition was calculated by
The system boundary between subsequent systems is defined
averaging Unilin's entire melamine faced fiberboard portfolio,
in accordance with EN 15804+A2, i.e. when the material
using the annual sales volumes as the weighting factor. The
reaches its end-of-waste state. End-of-life fiberboard reaches
raw board is manufactured at the Bazeilles and Vielsalm plants.
its end-of-waste state after a sorting and shredding step, as
The melamine faced board is produced at the SPANO and
inventoried in C3. The material leaves the current system at
BOSPAN sites. All of these production facilities are in the scope
module C3 and enters a subsequent system as a secondary
of this declaration.
fuel.
3.2 System boundary
3.3 Estimates and assumptions
This is a cradle-to-gate EPD with options, including the
Specific, primary data have been used to the highest extent
following life cycle phases A1 - A3, C1 - C4 and D. The
possible. In case of absence, estimates and assumptions were
following processes have been considered for each of the
made to model reality as closely as possible. These
modules:
assumptions are based on publicly available data and literature.
Generic dataset from the EcoInvent 3.8. database have been
A1 - A3: Product Stage
used to model the impact of some raw materials and process-
The production stage encompasses the extraction of raw
related parameters for which specific data was lacking.
materials (i.e. wood, paper, glue, resin, additives), their
transportation to the production plants, and the subsequent
End-of-life MDF board leaves the product system in C3 as a
manufacturing of the product. The required energy for
secondary fuel, for which the benefits and loads are inventoried
production, ancillary materials, and production emissions are
in module D. Here it is assumed that the secondary fuel
included. Energy and material input/output data were obtained
substitutes electricity and heat in accordance with an average
from Unilin's Bazeilles, Vielsalm, SPANO and BOSPAN plants
mix available on the European grid.
as well as its glue factory.
3.4 Cut-off criteria
A large share of the supplied production energy consists of All in- and outputs to the system under study have been
renewable energy, derived from non-recyclable woody waste included in the LCA. Primary data was used to the highest
streams. These waste streams are sourced in- and externally. extent possible. If primary data was lacking, secondary data
Unilin's fiberboard plants generate renewable thermal energy from EcoInvent was resorted to. Conservative assumptions
on-site. The biomass plants, A&S and A&U, produce renewable were made using average or generic data in case of data gaps.
energy from these woody waste streams, which is directly These assumptions are based on publicly available (literature
supplied to the SPANO and BOSPAN plants. Any remaining reported) data. As such, all processes, materials, or emissions
energy needs are met through the local grid in Belgium or expected to have a significant contribution to the environmental
France. impact of the system under study were considered in the LCA.
The total sum of omitted flows can therefore be deemed as
C1: Deconstruction/Demolition stage significantly below the 5 % threshold of the system's energy
It is assumed that the end-of-life melamine faced fiberboard is and mass input, as stated in the EN 15804+A2.
manually dismantled from the building/furniture. The efforts
involved in this process are considered negligible, leading to 3.5 Background data
the absence of a declared environmental impact arising from The relevant background data was either taken from the
the dismantling of the product. EcoInvent 3.8. database or peer-reviewed literature sources.
Measures were taken to ensure that the used secondary data
C2: Transport to Waste Processing was no more than 10 years old. These data types allowed to
This life cycle stage describes the impact of the end-of-life map the background system in the LCA of the product under
product's transport from the demolition site to the waste study.
processing facility. A representative distance of 50 km is
assumed. 3.6 Data quality
Data collection and necessary calculations were done in line
C3: Waste Processing with ISO 14044. Primary data was directly gathered from the
Processing of post-consumer MDF waste involves (preliminary) designated person at the relevant production plants. It was
sorting and shredding of the material. The fiberboard is ensured that the collected data accurately represented reality,
repurposed as a secondary fuel and undergoes energy so it can be assumed that the used primary data is of high
recovery in module D. The material and its inherent properties quality.
(e.g. biogenic carbon and primary energy content) are thus
5 Environmental Product Declaration - Unilin B.V. Division Panels - Unilin Melamine Faced MDF board
The technological, geographical, and time-related inherent material characteristics and underlying physical flows.
representativeness of background data (e.g. from EcoInvent) Fresh wood inventories were taken from EcoIvent 3.8. Here, it
was verified, as stated in EN 15804+A2. was made sure that the biogenic carbon and energy content
reflect the physical relationships of the different wood-based
3.7 Period under review materials.
Primary data, needed to calculate the LCA of the system under
study, was collected for the year 2020 from the Bazeilles, The system boundary (and subsequent allocation) relating to
Vielsalm, BOSPAN, SPANO and Unilin's glue production facility. the flow of the end-of-life product are as described in section
3.2.
3.8 Geographic Representativeness
Land or region, in which the declared product system is 3.10 Comparability
manufactured, used or handled at the end of the product´s Basically, a comparison or an evaluation of EPD data is only
lifespan: Belgium possible if all the data sets to be compared were created
according to EN 15804 and the building context, respectively
the product-specific characteristics of performance, are taken
3.9 Allocation
into account. Background data was used from the EcoInvent
In line with EN 15804+A2 and EN 16485, the biogenic carbon
3.8. database.
and primary energy content of the wood have been balanced
over the product's entire life cycle (A1 - C4) based on its
4. LCA: Scenarios and additional technical information
info.panels@unilin.com for more information.
Characteristic product properties of biogenic carbon
End-of-life (C1-C4)
The values declared below describe the amount of biogenic
The following table provides the parameters required to model
carbon and stored biogenic CO in the building product under
2 the end-of-life of the product under study. Since the product is
study when it leaves the factory gate. These relate to 1 m² of
not intended for extended outdoor use, it is assumed that its
Unilin melamine faced fiberboard, with a sales-weighted
moisture content remains consistent with its state at the factory
average composition and thickness (i.e. 15.9 mm).
gate. The end-of-life product reaches its end-of-waste state
Biogenic carbon content at factory gate after (preliminary) sorting and shredding. The losses during the
The carbon uptake of the packaging materials is not included sorting and shredding are assumed to have a negligible impact
below as their end-of-life impact is not declared in module A5. and are thus discarded. The material leaves the system as a
secondary fuel (energy recovery).
Name Value Unit
Biogenic carbon content in product 4.5 kg C/m² Name Value Unit
Stored carbon dioxide in product 16.3 kg CO2/m² Collected separately 11.24 kg/m²
Secondary fuel (output at C3) 11.24 kg/m²
Note: 1 kg biogenic carbon is equivalent to 44/12 kg CO .
2
Reuse, recovery and/or recycling potentials (D)
In module D, the loads and benefits of exporting the secondary
The following technical information is a basis for the declared
fuel from the system under study are inventoried. The moisture
modules or can be used for developing specific scenarios in the
content of this fuel is assumed to remain consistent with its
context of a building assessment if modules are not declared
state at factory gate. This value may vary significantly based on
(MND).
the storage conditions prior to its intended use.
Installation into the building (A5)
The end-of-life impact of the used packaging materials is not The recovery potential is modelled based on the net output flow
declared. However, its impact can be modelled based on the of secondary fuel. It is assumed that a biomass power plant
data given below. located in the EU recovers the secondary fuel's energy, with 55
% of the energy being recovered as heat and the remaining 30
Name Value Unit
% as electricity. The generated energy carriers are assumed to
Wood-based packaging 0.41 kg/m²
substitute heat and electricity in accordance with the average
Cardboard 0.004 kg/m² mix available on the European grid.
PET straps 0.0027 kg/m² Name Value Unit
Stretch foil 0.00067 kg/m² Net output flow of secondary fuel 10.49 kg/m²
Information on the reference lifetime can be found in section Energy efficiency biomass plant 85 %
2.12. Please contact Unilin's sales team or
6 Environmental Product Declaration - Unilin B.V. Division Panels - Unilin Melamine Faced MDF board
5. LCA: Results
The values declared below refer to 1 m² of Unilin melamine faced fiberboard with a sales-weighted average composition, grammage of
11.24 kg/m² and thickness of 15.9 mm.
Table "Description of the system boundary" summarizes the scope of the system under study from a life cycle point of view. Declared
modules are indicated with an "X", non-declared modules are indicated with "MND". "MNR" refers to modules which are deemed as not
relevant.
DESCRIPTION OF THE SYSTEM BOUNDARY (X = INCLUDED IN LCA; MND = MODULE OR INDICATOR NOT DECLARED; MNR
= MODULE NOT RELEVANT)
Benefits and
Construction loads beyond
Product stage Use stage End of life stage
process stage the system
boundaries
la ire ta m w a Ry lp p u s tro p s n a rT g n iru tc a fu n a M e h t m o rf tro p s n a rTe tis e h t o t e ta g y lb m e s s A e s U e c n a n e tn ia M ria p e R tn e m e c a lp e R tn e m h s ib ru fe R y g re n e la n o ita re p Oe s u re ta w la n o ita re p Oe s u n o itc u rts n o c -e Dn o itilo m e d tro p s n a rT g n is s e c o rp e ts a W la s o p s iD -e s u e R-y re v o c e R-g n ilc y c e Rla itn e to p
A1 A2 A3 A4 A5 B1 B2 B3 B4 B5 B6 B7 C1 C2 C3 C4 D
X X X MND MND MND MND MNR MNR MNR MND MND X X X X X
RESULTS OF THE LCA - ENVIRONMENTAL IMPACT according to EN 15804+A2: 1 m² Unilin Melamine Faced MDF Board
Parameter Unit A1-A3 C1 C2 C3 C4 D
Global Warming Potential total (GWP-total) kg CO 2 eq -1.26E+01 0 5.06E-02 1.65E+01 0 -9.64E+00
Global Warming Potential fossil fuels (GWP-fossil) kg CO 2 eq 3.64E+00 0 5.06E-02 1.9E-01 0 -9.6E+00
Global Warming Potential biogenic (GWP-biogenic) kg CO 2 eq -1.63E+01 0 1.57E-05 1.63E+01 0 -1.91E-02
Global Warming Potential luluc (GWP-luluc) kg CO 2 eq 2.14E-02 0 1.87E-05 2.58E-04 0 -1.45E-02
Depletion potential of the stratospheric ozone layer (ODP) kg CFC11 eq 6.78E-07 0 1.22E-08 2.73E-08 0 -1.36E-06
Acidification potential of land and water (AP) mol H+ eq 2.4E-02 0 2.13E-04 1.07E-03 0 -1.33E-02
Eutrophication potential aquatic freshwater (EP-freshwater) kg P eq 2.43E-04 0 3.49E-07 1.04E-05 0 -6.35E-04
Eutrophication potential aquatic marine (EP-marine) kg N eq 8.04E-03 0 6.43E-05 2.72E-04 0 6.48E-03
Eutrophication potential terrestrial (EP-terrestrial) mol N eq 8.18E-02 0 7.1E-04 3.04E-03 0 7.02E-02
Formation potential of tropospheric ozone photochemical oxidants kg NMVOC
3.11E-02 0 2.28E-04 8.62E-04 0 1.27E-02
(POCP) eq
Abiotic depletion potential for non fossil resources (ADPE) kg Sb eq 3.66E-05 0 1.21E-07 6.32E-07 0 -3.14E-06
Abiotic depletion potential for fossil resources (ADPF) MJ 1.1E+02 0 7.95E-01 3.43E+00 0 -2.5E+02
m3 world eq
Water use (WDP) 4.33E+00 0 2.69E-03 9.55E-03 0 -1.37E+00
deprived
RESULTS OF THE LCA - INDICATORS TO DESCRIBE RESOURCE USE according to EN 15804+A2: 1 m² Unilin Melamine
Faced MDF Board
Parameter Unit A1-A3 C1 C2 C3 C4 D
Renewable primary energy as energy carrier (PERE) MJ 9.3E+01 0 1.01E-02 1.71E+02 0 -2.06E+01
Renewable primary energy resources as material utilization
MJ 1.7E+02 0 0 -1.7E+02 0 0
(PERM)
Total use of renewable primary energy resources (PERT) MJ 2.63E+02 0 1.01E-02 3.65E-01 0 -2.06E+01
Non renewable primary energy as energy carrier (PENRE) MJ 8.02E+01 0 7.95E-01 3.25E+01 0 -2.5E+02
Non renewable primary energy as material utilization (PENRM) MJ 2.98E+01 0 0 -2.9E+01 0 0
Total use of non renewable primary energy resources (PENRT) MJ 1.1E+02 0 7.95E-01 3.43E+00 0 -2.5E+02
Use of secondary material (SM) kg 1.09E-03 0 0 0 0 0
Use of renewable secondary fuels (RSF) MJ 8.72E+00 0 0 0 0 1.35E+02
Use of non renewable secondary fuels (NRSF) MJ 0 0 0 0 0 2.3E+01
Use of net fresh water (FW) m3 1.24E-01 0 9.46E-05 1.91E-03 0 -1.01E-01
RESULTS OF THE LCA – WASTE CATEGORIES AND OUTPUT FLOWS according to EN 15804+A2:
1 m² Unilin Melamine Faced MDF Board
Parameter Unit A1-A3 C1 C2 C3 C4 D
Hazardous waste disposed (HWD) kg 1.89E-01 0 5.5E-04 5.12E-03 0 -2.5E-02
Non hazardous waste disposed (NHWD) kg 2.14E+00 0 7.84E-02 1.41E-01 0 -1.52E+00
Radioactive waste disposed (RWD) kg 6.82E-04 0 5.38E-06 2.4E-05 0 -9.93E-04
Components for re-use (CRU) kg 0 0 0 0 0 0
Materials for recycling (MFR) kg 0 0 0 0 0 0
Materials for energy recovery (MER) kg 0 0 0 1.12E+01 0 0
Exported electrical energy (EEE) MJ 0 0 0 0 0 0
Exported thermal energy (EET) MJ 0 0 0 0 0 0
7 Environmental Product Declaration - Unilin B.V. Division Panels - Unilin Melamine Faced MDF board
RESULTS OF THE LCA – additional impact categories according to EN 15804+A2-optional:
1 m² Unilin Melamine Faced MDF Board
Parameter Unit A1-A3 C1 C2 C3 C4 D
Disease
Incidence of disease due to PM emissions (PM) 2.68E-07 0 6E-09 1.26E-08 0 1.38E-07
incidence
Human exposure efficiency relative to U235 (IR) kBq U235 eq 5.29E-01 0 3.45E-03 2.35E-02 0 -1.14E+00
Comparative toxic unit for ecosystems (ETP-fw) CTUe 2.11E-05 0 9.73E-10 4.78E-09 0 -2.53E-08
Comparative toxic unit for humans (carcinogenic) (HTP-c) CTUh 2.44E-08 0 8.14E-12 5.32E-11 0 5.79E-10
Comparative toxic unit for humans (noncarcinogenic) (HTP-nc) CTUh 2.53E-09 0 2.48E-11 1.75E-10 0 -1.15E-09
Soil quality index (SQP) SQP 1.1E+03 0 9.1E-01 1.67E+00 0 -1.95E+01
Disclaimer 1 – for the indicator 'Potential Human exposure efficiency relative to U235'. This impact category deals mainly with the
eventual impact of low-dose ionizing radiation on human health of the nuclear fuel cycle. It does not consider effects due to possible
nuclear accidents, occupational exposure or radioactive waste disposal in underground facilities. Potential ionizing radiation from the
soil, radon and from some construction materials is also not measured by this indicator.
Disclaimer 2 – for the indicators 'abiotic depletion potential for non-fossil resources', 'abiotic depletion potential for fossil resources',
'water (user) deprivation potential, deprivation-weighted water consumption', 'potential comparative toxic unit for ecosystems', 'potential
comparative toxic unit for humans – cancerogenic', 'Potential comparative toxic unit for humans - not cancerogenic', 'potential soil
quality index'. The results of this environmental impact indicator shall be used with care as the uncertainties on these results are high
as there is limited experience with the indicator.
6. LCA: Interpretation
This section aims to analyze and interpret the results of the and stores it as biogenic carbon in its biomass. The product's
LCA analysis carried for 1 m² of the Unilin melamine faced MDF high wood content (i.e. 80 %) results in a GWP-total of - 12.6
board. The results shown below refer to the product with a kg/m². The product thus stores carbon and does not contribute
sales-weighted average composition and thickness (15.9 mm). to global warming when it leaves Unilin's factory gate. The
Although the values for specific commercial references and stored carbon will only be released if the fiberboard can no
thicknesses can vary from the declared and discussed ones, longer fulfill its intended purpose (i.e. at end of life).
the observed trends will be the same throughout the entire
product category. A deep dive in the drivers of the cradle-to-gate environmental
impact shows the significant contribution of the raw materials
Summary (module A1). 67 % of the fossil CO emissions can primarily be
2
This part intends to summarize the trends observed in the allocated to the glue and resin production, as well as 90 % of
cradle-to-gate environmental impact of the Unilin melamine the water used in A1 - A3. The generation of heat and
faced fiberboard. An in-depth analysis is available in the electricity, required for the melamine faced MDF production, is
following subsections. an important driver of the production-related impact. This is
observable in the EP-m and POCP indicators.
During its growth, wood absorbs CO through photosynthesis
2
Wood stores CO as biogenic carbon during its growth (GWP-
2
Cradle-to-Cradle Impact - Dominance Analysis biogenic = - 16.3 kg CO eq./m²). This negative GWP-value is
2
The hot-spot analysis highlights the negative GWP-value of
partially counterbalanced by the positive GWP-impact of the
modules A1 - A3, as depicted in the GWP-focused graph. To
fossil materials and energy resources used during A1 - A3
improve the clarity of the graph, the values of the GWP-luluc
(GWP-fossil). This results in a GWP-total of - 12.6 kg CO
indicator have been omitted. 2
eq./m² when the Unilin melamine faced MDF board leaves the
factory gate. The product under study thus stores carbon and
8 Environmental Product Declaration - Unilin B.V. Division Panels - Unilin Melamine Faced MDF board
does not contribute to global warming. fossil-based, a negative GWP-fossil is obtained (i.e. avoided
fossil CO emissions from combustion). It indicates that the
2
The stored carbon will only be released when the fiberboard combustion of these fossil fuels has a higher impact on global
leaves the system as a secondary fuel. The figure below clearly warming than the energy recovery from the secondary fuel.
demonstrates a neutral biogenic carbon balance in accordance
with EN 16485. The hot-spot analysis shows that, for non-GWP-related
parameters, modules A1 - A3 are the main contributors to the
The GWP-focused analysis also illustrates the "avoided" impact system under study. Values for module D are generally
(described in module D) related to the export of end-of-life negative, except for the EP and POCP indicators. This is
fiberboard as a secondary fuel. The energy recovery of that fuel attributed to the emissions from the energy recovery process of
generates heat and electricity, which substitutes a European the end-of-life fiberboard.
averaged mix of heat and electricity from the grid. Since the
largest share of the heat and electricity on the European grid is
indicators ODP, ADPE and WDP. 90 % of all water used in
Cradle-to-Grave Impact - Main Drivers modules A1 - A3 is allocated to the production of the raw
The graph below allows to identify the primary sources of the materials (mainly related to the glue and resin production).
cradle-to-gate environmental impact. The results show that raw
material production (module A1) has a significant impact. 67 % Energy-related processes are typically the main drivers of the
of the fossil CO emissions are primarily attributed to the environmental impact of module A3. This is observed in the
2
production of the used glue and resin. The contribution of the contribution of A3 to EP and POCP, which is traced back to the
raw material production is even more significant for the generation of renewable energy from woody waste.
9 Environmental Product Declaration - Unilin B.V. Division Panels - Unilin Melamine Faced MDF board
7. Requisite evidence
Formaldehyde emissions
AFFSET - Arrêté du 19 avril 2011 (28 days [Class])
E1 - EN 13986:2004+A1:2015 • Test Report : 402-21-1109C-3-f-e
• Method : ISO 16000
• Test report : 1110
• Product : Melamine Faced MDF
• Method : EN 717-1
• Laboratory : FCBA
• Product : Melamine Faced MDF
Name Value Unit
• Laboratory : TCNH
Formaldehyde A+ Class
• Result : 0.01 ppm [Limit < 0.1 ppm]
Acetaldehyde A+ Class
E0.5 - ChemVerbotsV Toluene A+ Class
• Test report : 1110 Tetrachloroethylene A+ Class
• Method : EN 717-1 Xylene A+ Class
• Product : Melamine Faced MDF 1,2,3- Trimethylbenzene A+ Class
• Laboratory : TCNH
1,4-dichlorobenzene A+ Class
• Result : 0.01 ppm [Limit < 0.05 ppm]
Ethylbenzene A+ Class
PCP + Heavy metals + Wood preservative analysis
2-Butoxyethanol A+ Class
Styrene A+ Class
As the Unilin melamine faced fiberboard does not contain any
post-consumer COVT fid A+ Class
recycled wood, this evidence is not necessary.
VOC Emissions
Melamine faced fiberboards are commonly used for interior
building. In many countries national regulations are applicable
for indoor air quality. For other indoor air analysis reports
please contact Unilin's sales team or info.panels@unilin.com
for more information.
German AgBB (2021) overview of results (28 days [µg/m³])
• Test Report : ML01911-10R
• Method : ISO 16516
• Product : Melamine Faced Fibromax
• Laboratory : Servaco Product Testing
Name Value Unit
TVOC (C6 - C16) < 1000 μg/m3
Sum SVOC (C16 - C22) < 100 μg/m3
R (dimensionless) < 1 -
VOC without NIK < 100 μg/m3
Carcinogenic Substances < 1 μg/m3
10 Environmental Product Declaration - Unilin B.V. Division Panels - Unilin Melamine Faced MDF board
8. References
Standards
EN 13986
ASTM D6007
EN 13986:2004+A1:2015, Wood-based panels for use in
ASTM D6007:2020, Standard Test Method for Determining construction— Characteristics, valuation of conformity and
Formaldehyde Concentrations in Air from Wood Products Using marking
a Small-Scale Chamber
EN 14322
ASTM E1333
EN 14322:2021, Wood-based panels - Melamine faced boards
ASTM E1333:2020, Standard Test Method for Determining for interior uses - Definition, requirements and classification.
Formaldehyde Concentrations in Air and Emission Rates from
Wood Products Using a Large Chamber. EN 15804
EN 310 EN 15804:2012+A2:2019+AC:2021, Sustainability of
construction works — Environmental Product Declarations —
EN 310:1993, Wood-based panels - Determination of modulus Core rules for the product category of construction products.
of elasticity in bending and of bending strength.
EN 16000 - 3
EN 311
EN 16000 - 3: 2011, Air sampting on DNPH cartidge and
EN 311:2002, Wood-based panels - Surface soundness - Test analysis of Iow molecularweight carbonyl compounds by
method. HPLC/UV
EN 319 EN 16000 - 6
EN 319:1993, Particleboards and fibreboards - Determination EN 16000 - 6: 2012, Air sampling on multiadsorbent (Tenax TA /
of tensile strength perpendicular to the plane of the board gtass wool) and analysis of volatile organic compounds (VOC)
by TD/cCmS/FID
EN 322
EN 16000 - 9
EN 322:1993, Wood-based panels - Determination of moisture
content. EN 16000 - 9: 2006, lndoor air - Paft 9: Determination of the
emission of volatile organic compounds from building products
EN 323 and furnishing - Emission test chamber method
EN 323:2005, Wood-based panels - Determination of density. EN 16000 - 11
EN 324 EN 16000 - 11: 2006, Indoor air — Part 11: Determination of the
emission of volatile organic compounds from building products
EN 324-1:1993, Wood-based panels - Determination of and furnishing — Sampling, storage of samples and
dimensions of boards - Part 1: Determination of thickness, preparation of test specimens.
width and length.
EN 16449
EN 622
EN 16449:2014, Wood and wood-based produts - Calculation
EN 622-5:2010, Fibreboards - Specifications - Part 5: of the biogenic carbon content of wood and conversion to
Requirements for dry process boards (MDF). carbon dioxide.
EN 717-1 EN 16485
EN 717-1:2004, Wood-based panels - Determination of EN 16485:2014, Round and sawn timber. Environmental
formaldehyde release Formaldehyde emission by the chamber Product Declarations. Product category rules for wood and
method. wood-based products for use in consruction.
EN 12460-5 EN 16516
EN 12460-5:2015, Wood-based panels. Determination of EN 16516:2020, Construction products: Assessment of release
formaldehyde release Extraction method (called the perforator of dangerous substances - Determination of emissions into
method). indoor air.
EN 13501-1 ISO 9001
EN 13501-1:2007-05+A1:2009, Fire classification of EN ISO 9001:2008-11, Quality Management Systems –
construction products and building elements - Part 1: Requirements
classification with the results of tests on the reaction to fire of
building products.
11 Environmental Product Declaration - Unilin B.V. Division Panels - Unilin Melamine Faced MDF board
ISO 14001 for marketing building products.
EN ISO 14001:2015, Environmental management systems — EcoInvent 3.8.
Requirements with guidance for use.
Ecoinvent 3.8, Database for Life Cycle Inventory and
ISO 14025 Assessment. Swiss Centre for Life Cycle Inventories, 2021.
EN ISO 14025:2011, Environmental labels and declarations — Available at: https://ecoinvent.org/the-ecoinvent-database/data-
Type III environmental declarations — Principles and releases/ecoinvent-3-8/.
procedures.
EU Biocidal Products Ordinance No. 528/2012
ISO 14040
Regulation (EU) No 528/2012 of the European Parliament and
EN ISO 14040:2006-10, Environmental management — Life Council of 22 May 2012 concerning the making available on the
cycle assessment — Principles and framework. market and use of biocidal products.
ISO 14044 EWC
ISO 14044:2006-10, Environmental management — Life cycle European Waste Catalogue, Ordinance on the European Waste
assessment — Principles and framework. Catalogue (Waste Catalogue Ordinance - AVV), reference
Federal Official Journal I 2001, 3379.
ISO 45001
IBU 2022
EN ISO 45001:2018, Occupational health and safety
management systems — Requirements with guidance for use. Institut Bauen und Umwelt e.V.: General Instructions for the
EPD programme of Institut Bauen und Umwelt e.V., Version
ISO 50001 2.1, Berlin: Institut Bauen und Umwelt e.V., 2022
www.ibu-epd.com.
EN ISO 50001:2018, Energy management systems —
Requirements with guidance for use. PCR Part A
JIS A 1460 Product Category Rules for Building-Related Products and
Services. Part A: Calculation Rules for the Life Cycle
JIS A 1460:2021, Building boards Determination of Assessment and Requirements on the Project Report according
formaldehyde emission -- Desiccator method. to EN 15804+A2:2019. Version 1.3. Berlin: Institut Bauen und
Umwelt e.V. (eds.), 2021.
JIS A 5908
PCR Part B
JIS A 5908:2022, Particleboards.
Product Category Rules for Building-Related Products and
Additional References Services. Part B: Requirements on the EPD for Wood based
panels. Version 2. Berlin: Institut Bauen und Umwelt e.V. (eds.),
BBSR Table 2023.
BBSR 2017, Useful lives of building components for life cycle
analyses according to the Sustainable Building Assessment SVHC List
System, 2017, BBSR Germany 2017.
CPR List of Substances of Very High Concern (SVHC) Candidate for
Authorisation (ECHA Candidate List), dated 04.07.2023,
CPR EU Ordinance No. 305/2011 of the European Parliament published in accordance with Article 59(10) of the REACH
and Council of 9th March 2011 to define harmonized conditions Regulation. Helsinki: European Chemicals Agency.
12 Environmental Product Declaration - Unilin B.V. Division Panels - Unilin Melamine Faced MDF board
Publisher
Institut Bauen und Umwelt e.V. +49 (0)30 3087748- 0
Hegelplatz 1 info@ibu-epd.com
10117 Berlin www.ibu-epd.com
Germany
Programme holder
Institut Bauen und Umwelt e.V. +49 (0)30 3087748- 0
Hegelplatz 1 info@ibu-epd.com
10117 Berlin www.ibu-epd.com
Germany
Author of the Life Cycle Assessment
Unilin B.V. Division Panels +32 56 67 52 11
Ooigemstraat 3 info.panels@unilin.com
8710 Wielsbeke https://www.unilinpanels.com/en-
Belgium gb
Owner of the Declaration
Unilin B.V. Division Panels +32 56 66 70 21
Ooigemstraat 3 info.panels@unilin.com
8710 Wielsbeke https://www.unilinpanels.com/en-
Belgium gb
13 Environmental Product Declaration - Unilin B.V. Division Panels - Unilin Melamine Faced MDF board
