ENVIRONMENTAL PRODUCT DECLARATION
as per ISO 14025 and EN 15804+A2
Owner of the Declaration SOLBET SP. Z O.O.
Publisher Institut Bauen und Umwelt e.V. (IBU)
Programme holder Institut Bauen und Umwelt e.V. (IBU)
Declaration number EPD-SOL-20230257-CBD1-EN
Issue date 24/10/2023
Valid to 23/10/2028
Autoclaved Aerated Concreate (AAC)
Solbet Sp. z o.o.
www.ibu-epd.com | https://epd-online.com
General Information
Solbet Sp. z o.o. Autoclaved Aerated Concreate (AAC)
Programme holder Owner of the declaration
IBU – Institut Bauen und Umwelt e.V. SOLBET SP. Z O.O.
Hegelplatz 1 Torunska 71
10117 Berlin 86-050 Solec Kujawski
Germany Poland
Declaration number Declared product / declared unit
EPD-SOL-20230257-CBD1-EN 1 m3 of non-reinforced SOLBET autoclaved aerated concrete (AAC) with
the average density per product with moisture content declared at factory
gate is 663 kg/m3. The average gross density (dry mass) of the declared
product is 515 kg/m3.
This declaration is based on the product category rules: Scope:
Aereated Concrete, 01/08/2021 The LCA is based on consideration on all SOLBET Group plants:
(PCR checked and approved by the SVR)
SOLBET Sp. z o.o.:
• Solec Kujawski plant,
Issue date
• Podnieśno plant,
24/10/2023 • Rurka plant,
SOLBET LUBARTÓW S.A.:
Valid to • Lubartów plant,
23/10/2028
SOLBET KOLBUSZOWA S.A.:
• Głogów Małopolski plant,
• Lipie plant,
SOLBET STALOWA WOLA S.A.:
• Stalowa Wola plant,
and the data basis is 2021.
The owner of the declaration shall be liable for the underlying information
and evidence; the IBU shall not be liable with respect to manufacturer
information, life cycle assessment data and evidences.
Dipl.-Ing. Hans Peters
(Chairman of Institut Bauen und Umwelt e.V.) The EPD was created according to the specifications of EN 15804+A2. In
the following, the standard will be simplified as EN 15804.
Verification
The standard EN 15804 serves as the core PCR
Independent verification of the declaration and data according to ISO
14025:2011
internally X externally
Florian Pronold Mrs Kim Allbury,
(Managing Director Institut Bauen und Umwelt e.V.) (Independent verifier)
1 Environmental Product Declaration - Solbet Sp. z o.o. - Autoclaved Aerated Concreate (AAC)
Product
Specification for masonry units - Part 4: Autoclaved aerated
Product description/Product definition concrete masonry unit.
The subject of the declaration are non-reinforced aerated
concrete masonry elements of various sizes and density Base materials/Ancillary materials
classes, manufactured using the autoclaving process. SOLBET Name Value Unit
products are used to construct load-bearing and non-
Sand 40 - 85 M, %
loadbearing masonry structures in all types of walls, including
Water 40 - 80 M, %
single leaf, cavity, partitions, retaining, basement and external
Cement 10 - 50 M, %
walls with a covered facing surface. Elements of autoclaved
aerated concrete should be classified as an lightweight Lime 5 - 45 M, %
concrete. Gypsum 0 - 10 M, %
Aluminium powder 0.01 - 0.15 M, %
SOLBET autoclaved aerated concrete (AAC) elements are
produced according to EN 771-4:2011+A1:2015 - Specification Sand: sand is the basic raw material necessary for the reaction
for masonry units - Part 4: Autoclaved aerated concrete in the hydrothermal process. The sands used are of natural
masonry units. All Autoclaved Aerated Concrete elements in origin, mainly composed of quartz dioxide (SiO2).
SOLBET group are produced in system 2+ in Category I in Water: Water is essential for the chemical processes involved
accordance with EN 771-4. All AAC products produced in in the production of aerated concrete. Water is also used for
SOLBET group have DoP according to regulation 305/2011 and grinding, and for obtaining steam in the autoclaving process.
the CE market. Cement: in accordance with the standard EN 197-1:2011,
Cement is used as a binder. It is formed as a result of burning
Autoclaved Aerated Concrete in SOLBET group is produced natural rocks, e.g. marl and limestone.
according to EN 771-4:2011+A1:2015 definition: the AAC is Lime: in accordance with the standard EN 459-1:2015, Lime is
"manufactured from hydraulic binders such as cement and/or used as a binder. It is formed as a result of burning natural
lime, combined with siliceous based fine material, cell limestone rocks.
generating material and water and cured with high pressure Gypsum: Gypsum of natural origin or from flue gas
steam in autoclaves". desulfurization in power plants is used. It acts as a regulator of
For the placing on the market of the product in the European setting time and takes part in reactions in the hydrothermal
Union/European Free Trade Association (EU/EFTA) (with the process.
exception of Switzerland) Regulation (EU) No. 305/2011 (CPR) Aluminium powder: in accordance with the polish standard
applies. The product needs a declaration of performance taking PN-H-97021:1998 - polish version, Aluminum powder emitting
into consideration EN 771-4:2011+A1:2015, Specification for hydrogen in an alkaline environment causes the formation of a
masonry units - Part 4: Autoclaved aerated concrete masonry porous structure of autoclaved aerated concrete.
unit and the CE-marking. For the application and use the
respective national provisions 1) This product / article / at least one partial article contains
apply. substances listed in the candidate list Candidate List of
substances of very high concern exceeding 0.1 percentage by
Application mass: No.
Autoclaved aerated concrete elements are using in all kinds of 2) This product /article /at least one partial article contains other
construction and non-construction walls: single-layer wall, multi- CMR substances in categories 1A or 1B which are not on the
layer wall, cavity wall, retaining wall and basements, and in all candidate list, exceeding 0.1 percentage by mass: No.
external elements with a protected face surface. 3) Biocide products were added to this construction product or it
has been treated with biocide products (this then concerns a
Technical Data treated product as defined by the (EU) Ordinance on Biocide
The basic functional properties of wall elements made of Products No. 528/2012): No.
autoclaved aerated concrete, produced in the SOLBET capital
group, are presented in the table below. Reference service life
Autoclaved aerated concrete (AAC) is a durable material. Walls
Constructional Data
constructed from the products will fulfill their intended function
Name Value Unit for the life of the building in which they have been installed.
Compressive strength (according to EN 772- AAC is the most popular building material in Poland from many
1+A1:2015-10, p. 7.3.4. Tested on cubes 100 1.5 - 5 N/mm2 years. Tradition of using AAC in Poland has more than 70
mm) years, and existing buildings still are using without any
Gross density (dry density, according to EN 300 - problems - without any plasters or other surface protect.
kg/m3
772-13)) 710 Aerated concrete recarbonates naturally and thus absorbs
atmospheric CO during its service life. The essential properties
0.08 - 2
Thermal conductivity (according to EN 1745) W/(mK)
0.18 such as thermal conductivity and strength of aerated concrete
do not change as a result after leaving the autoclave.
Water vapour diffusion resistance factor
5 -
(according to EN 1745)
The Reference Service Life (RSL) of AAC is connected with
Shrinkage (according to EN 680. Reference
0.4 mm/m properties of AAC. The reference service life is 150 years
value not higher than declared value)
based on Roadmap for AAC, conference paper from 7th ICAAC
Performance data of the product in accordance with the in Prague, and tests of existing buildings.
declaration of performance with respect to its essential
characteristics according to EN 771-4:2011+A1:2015,
2 Environmental Product Declaration - Solbet Sp. z o.o. - Autoclaved Aerated Concreate (AAC)
LCA: Calculation rules
the building context and can be estimated approximately via the
Declared Unit declared values for the production stage.
The declared unit is 1 m3 of non-reinforced aerated concrete. The installation of the products themselves is usually done
The average density per product with moisture content manually (load-free).
declared at factory gate is 663 kg/m3. The average density
according to EN 771-4:2011+A1:2015 in dry mass is 515 kg/m3. Use stage (B1)
Carbonation of reactive product components (e.g. CaO and
Declared unit and mass reference
MgO) are considered in this module. A carbonation rate of
Name Value Unit 98.97 % is assumed, P. Walczak / SOLBET Research Center
Declared unit 1 m3 Department, 2022.
Gross density 663 kg/m3
End-of-life stage– Modules C1-C4
Dry density (according to EN 772-13) 515 kg/m3
The end-of-life stage includes:
As an estimate of the robustness of the LCA values, the • Module C1: Mechanical dismantling (excavator).
weighted average density of the declared AAC product is • Module C2: Truck transport to EoL (50km). If necessary,
calculated relative to the production volume shares of the transport distance can be adapted to building level.
seven production sites in scope located across Poland. The • Module C3: Construction waste processing (shredding)
production process remains the same across all sites in scope. and material recycling as filling material (incl. credits for
All background datasets relevant for the production of the substitution of gravel in Module D) assuming 5 %
declared of AAC product were mapped to technologically recycling losses are sent to landfill. The end of waste
similar upstream processes from the Sphera LCA FE (GaBi ts) status is reached after shredding. This module also
software and databases. considers carbonation at the end of life.
System boundary
Reuse, recovery or recycling potential beyond system
Type of EPD according to EN 15804: cradle to gate with
boundary - Module D
options, modules C1–C4, and module D.
This module considers material credits from saved
The following modules are declared: A1–A3, C, D and
expenditures through the substitution of gravel as backfill
additional modules: A4 + A5 +B1.
material (module C3).
It also includes the credits of the thermal and electrical energy
Production - Modules A1-A3
generated in Module A5 due to the thermal treatment of
The product stage includes:
packaging. Avoided burdens have been calculated by the
• Raw material supply (A1) inversion of residual grid mix and thermal energy from natural
• Transport to the manufacturer (A2) gas, using European datasets.
• Manufacturing (A3), including provision of all
materials, products and energy, as well as waste Geographic Representativeness
processing up to the end-of-waste state. Packaging is Land or region, in which the declared product system is
also considered in this module. manufactured, used or handled at the end of the product´s
lifespan: Poland
Construction stage - Modules A4-A5
The construction process stage includes:
Comparability
• Transport to the construction site (A4): This module
Basically, a comparison or an evaluation of EPD data is only
considers 100 km truck transport to the site. The
possible if all the data sets to be compared were created
transport distance can be modified project-specific if
according to EN 15804 and the building context, respectively
required by linear scaling.
the product-specific characteristics of performance, are taken
• Thermal treatment of packaging material (A5) where the
into account.
resulting credits are declared in module D.
Background database: Sphera LCA FE (GaBi ts), CUP2022.1
Offcuts were not taken into account, as they strongly depend on
LCA: Scenarios and additional technical information
Characteristic product properties of biogenic carbon Note: 1 kg of biogenic carbon is equivalent to 44/12 kg of CO .
2
No biogenic carbon is reported in the product. The biogenic
carbon content in the accompanying packaging for 1 m3 of non-
reinforced aerated concrete is declared below. The following technical scenario information is required for the
Information on describing the biogenic carbon content at declared modules and optional for non-declared modules.
factory gate The following technical information is a basis for the declared
modules or can be used for developing specific scenarios in the
Name ValueUnit
context of a building assessment if modules are not declared
kg
Biogenic carbon content in product - (MND).
C
The values refer to the declared unit of 1 m3 of non-reinforced
Biogenic carbon content in accompanying kg
1.11 aerated concrete.
packaging C
3 Environmental Product Declaration - Solbet Sp. z o.o. - Autoclaved Aerated Concreate (AAC)
Transport to the building site (A4) Reference service life
Name Value Unit
Name Value Unit Life Span according to the manufacturer 150 a
Litres of fuel 1.31 l/100km
End of life (C1-C4)
Transport distance 100 km
The values refer to the declared unit of 1 m3 of non-reinforced
Capacity utilisation (including empty runs) 61 %
aerated concrete.
Gross density of packed product transported 666 kg/m3
Name ValueUnit
The transport distance can be modified to project-specific
Diesel consumption for mechanical dismantling via
criteria if required by linear scaling. 0.114 kg
excavator (Module C1)
Collected separately waste type waste type 663 kg
Installation into the building (A5)
Recycling 630 kg
The thermal treatment of the packaging is considered in
Landfilling 33 kg
module A5. The following quantities are scaled per m3 of non-
reinforced aerated concrete. Reuse, recovery and/or recycling potentials (D), relevant
scenario information
Name ValueUnit
Wooden pallet packaging to incineration (weighted
2.96 kg Module D includes the material credits from saved expenditures
average based on production volume shares)
through substitution of gravel as backfill material (module C3).
Polyethylene foil packaging to incineration It also includes the credits of the thermal and electrical energy
(weighted average based on production volume 0.45 kg generated in Module A5 due to the thermal treatment of
shares) packaging. Avoided burdens have been calculated by the
inversion of residual grid mix and thermal energy from natural
Use or application of the installed product (B1) see section
gas, using European datasets.
2.12 "Use"
A waste incineration plant with R1-value > 0.6 is assumed.
Name ValueUnit
Carbonation rate (P. Walczak, SOLBET Research
98.97 %
Center Department, 2022)
4 Environmental Product Declaration - Solbet Sp. z o.o. - Autoclaved Aerated Concreate (AAC)
LCA: Results
The following tables display the environmentally relevant results according to EN 15804 for 1 m3 of non-reinforced aerated concrete.
The average density per product with moisture content declared at factory gate is 663 kg/m3.
DESCRIPTION OF THE SYSTEM BOUNDARY (X = INCLUDED IN LCA; MND = MODULE OR INDICATOR NOT DECLARED; MNR
= MODULE NOT RELEVANT)
Benefits and
Construction loads beyond
Product stage Use stage End of life stage
process stage the system
boundaries
la ire ta m w a Ry lp p u s tro p s n a rT g n iru tc a fu n a M e h t m o rf tro p s n a rTe tis e h t o t e ta g y lb m e s s A e s U e c n a n e tn ia M ria p e R tn e m e c a lp e R tn e m h s ib ru fe R y g re n e la n o ita re p Oe s u re ta w la n o ita re p Oe s u n o itc u rts n o c -e Dn o itilo m e d tro p s n a rT g n is s e c o rp e ts a W la s o p s iD -e s u e R-y re v o c e R-g n ilc y c e Rla itn e to p
A1 A2 A3 A4 A5 B1 B2 B3 B4 B5 B6 B7 C1 C2 C3 C4 D
X X X X X X MND MNR MNR MNR MND MND X X X MND X
RESULTS OF THE LCA - ENVIRONMENTAL IMPACT according to EN 15804+A2: 1 m3 non-reinforced AAC product
Parameter Unit A1-A3 A4 A5 B1 C1 C2 C3 D
GWP-total kg CO 2 eq 1.66E+02 4.02E+00 5.93E+00 -7.52E+01 4.28E-01 2E+00 1.44E+00 -3.81E+00
GWP-fossil kg CO 2 eq 1.7E+02 3.98E+00 1.49E+00 -7.52E+01 4.26E-01 1.98E+00 1.43E+00 -3.82E+00
GWP-biogenic kg CO 2 eq -4.35E+00 1.68E-02 4.44E+00 0 1.98E-10 8.37E-03 3.21E-04 2.13E-02
GWP-luluc kg CO 2 eq 4.89E-02 2.22E-02 1.16E-05 0 2.27E-03 1.11E-02 8.85E-03 -3.51E-03
ODP kg CFC11 eq 1.19E-10 2.39E-13 4.62E-13 0 2.44E-14 1.19E-13 3.71E-12 -1.96E-11
AP mol H+ eq 3.11E-01 3.8E-03 8.97E-04 0 2.02E-03 1.89E-03 1.24E-02 -9.07E-03
EP-freshwater kg P eq 5.98E-05 1.19E-05 1.1E-07 0 1.22E-06 5.92E-06 5.76E-06 -6.41E-06
EP-marine kg N eq 9.48E-02 1.18E-03 2.77E-04 0 9.5E-04 5.89E-04 4.94E-03 -3.07E-03
EP-terrestrial mol N eq 1.04E+00 1.42E-02 4.26E-03 0 1.05E-02 7.07E-03 5.45E-02 -3.38E-02
kg NMVOC
POCP 2.74E-01 3.31E-03 7.6E-04 0 2.67E-03 1.65E-03 1.37E-02 -8.52E-03
eq
ADPE kg Sb eq 9.38E-06 3.34E-07 1.13E-08 0 3.41E-08 1.66E-07 1.95E-06 -4.3E-07
ADPF MJ 1.07E+03 5.33E+01 1.27E+00 0 5.45E+00 2.65E+01 4E+01 -6.61E+01
m3 world eq
WDP 2.92E+00 3.58E-02 6.85E-01 0 3.65E-03 1.78E-02 3.85E-01 -2.42E-01
deprived
GWP = Global warming potential; ODP = Depletion potential of the stratospheric ozone layer; AP = Acidification potential of land and water; EP =
Eutrophication potential; POCP = Formation potential of tropospheric ozone photochemical oxidants; ADPE = Abiotic depletion potential for non-fossil
resources; ADPF = Abiotic depletion potential for fossil resources; WDP = Water (user) deprivation potential)
RESULTS OF THE LCA - INDICATORS TO DESCRIBE RESOURCE USE according to EN 15804+A2: 1 m3 non-reinforced AAC
product
Parameter Unit A1-A3 A4 A5 B1 C1 C2 C3 D
PERE MJ 1.11E+02 3.03E+00 4.4E+01 0 3.1E-01 1.51E+00 3.67E+00 -9.61E+00
PERM MJ 4.37E+01 0 -4.37E+01 0 0 0 0 0
PERT MJ 1.54E+02 3.03E+00 2.96E-01 0 3.1E-01 1.51E+00 3.67E+00 -9.61E+00
PENRE MJ 1.05E+03 5.34E+01 2.2E+01 0 5.46E+00 2.66E+01 4.01E+01 -6.61E+01
PENRM MJ 2.07E+01 0 -2.07E+01 0 0 0 0 0
PENRT MJ 1.07E+03 5.34E+01 1.27E+00 0 5.46E+00 2.66E+01 4.01E+01 -6.61E+01
SM kg 5.58E+00 0 0 0 0 0 0 0
RSF MJ 0 0 0 0 0 0 0 0
NRSF MJ 0 0 0 0 0 0 0 0
FW m3 1.53E-01 3.43E-03 1.61E-02 0 3.5E-04 1.71E-03 1.1E-02 -1.19E-02
PERE = Use of renewable primary energy excluding renewable primary energy resources used as raw materials; PERM = Use of renewable primary
energy resources used as raw materials; PERT = Total use of renewable primary energy resources; PENRE = Use of non-renewable primary energy
excluding non-renewable primary energy resources used as raw materials; PENRM = Use of non-renewable primary energy resources used as raw
materials; PENRT = Total use of non-renewable primary energy resources; SM = Use of secondary material; RSF = Use of renewable secondary fuels;
NRSF = Use of non-renewable secondary fuels; FW = Use of net fresh water
RESULTS OF THE LCA – WASTE CATEGORIES AND OUTPUT FLOWS according to EN 15804+A2:
1 m3 non-reinforced AAC product
Parameter Unit A1-A3 A4 A5 B1 C1 C2 C3 D
HWD kg 2.28E-05 2.56E-10 1.23E-10 0 2.61E-11 1.27E-10 7.53E-10 -6.62E-09
NHWD kg 1.7E+01 7.66E-03 4.41E-02 0 7.82E-04 3.81E-03 3.32E+01 -2.62E+01
RWD kg 2.24E-02 6.58E-05 7.56E-05 0 6.72E-06 3.27E-05 5.15E-04 -5.68E-03
CRU kg 0 0 0 0 0 0 0 0
MFR kg 0 0 0 0 0 0 6.3E+02 0
MER kg 0 0 0 0 0 0 0 0
EEE MJ 0 0 1.08E+01 0 0 0 0 0
5 Environmental Product Declaration - Solbet Sp. z o.o. - Autoclaved Aerated Concreate (AAC)
EET MJ 0 0 1.93E+01 0 0 0 0 0
HWD = Hazardous waste disposed; NHWD = Non-hazardous waste disposed; RWD = Radioactive waste disposed; CRU = Components for re-use;
MFR = Materials for recycling; MER = Materials for energy recovery; EEE = Exported electrical energy; EET = Exported thermal energy
RESULTS OF THE LCA – additional impact categories according to EN 15804+A2-optional:
1 m3 non-reinforced AAC product
Parameter Unit A1-A3 A4 A5 B1 C1 C2 C3 D
Disease
PM 4.56E-06 2.3E-08 4.54E-09 0 2.28E-08 1.14E-08 2.11E-07 -4E-07
incidence
IR kBq U235 eq 3.77E+00 9.65E-03 1.24E-02 0 9.85E-04 4.8E-03 8.04E-02 -8.58E-01
ETP-fw CTUe 3.98E+02 3.7E+01 5.66E-01 0 3.78E+00 1.84E+01 2.6E+01 -1.9E+01
HTP-c CTUh 1.99E-08 7.46E-10 4.23E-11 0 7.62E-11 3.71E-10 1.04E-09 -1.12E-09
HTP-nc CTUh 1.86E-06 3.86E-08 1.44E-09 0 4.62E-09 1.92E-08 8.71E-08 -9.66E-08
SQP SQP 7.83E+02 1.83E+01 3.78E-01 0 1.87E+00 9.13E+00 8.93E+00 -8.14E+00
PM = Potential incidence of disease due to PM emissions; IR = Potential Human exposure efficiency relative to U235; ETP-fw = Potential comparative
Toxic Unit for ecosystems; HTP-c = Potential comparative Toxic Unit for humans (cancerogenic); HTP-nc = Potential comparative Toxic Unit for humans
(not cancerogenic); SQP = Potential soil quality index
Disclaimer 1 – for the indicator “Potential Human exposure efficiency relative to U235”. This impact category deals mainly with the
eventual impact of low-dose ionizing radiation on human health of the nuclear fuel cycle. It does not consider effects due to possible
nuclear accidents, occupational exposure or radioactive waste disposal in underground facilities. Potential ionizing radiation from the
soil, radon and from some construction materials is also not measured by this indicator.
Disclaimer 2 – for the indicators “abiotic depletion potential for non-fossil resources”, “abiotic depletion potential for fossil resources”,
“water (user) deprivation potential, deprivation-weighted water consumption”, “potential comparative toxic unit for ecosystems”,
“potential comparative toxic unit for humans – cancerogenic”, “Potential comparative toxic unit for humans - not cancerogenic”,
“potential soil quality index”. The results of this environmental impact indicator shall be used with care as the uncertainties on these
results are high as there is limited experience with the indicator.
References
Standards
CPR
EN 197-1 REGULATION (EU) No 305/2011 OF THE EUROPEAN
EN 197-1:2011, Cement Composition, specifications and PARLIAMENT AND OF THE COUNCIL
conformity criteria for common cements of 9 March 2011. Laying down harmonised conditions for the
marketing of construction products and repealing Council
EN 459-1 Directive 89/106/EEC
EN 459-1:2015, Building lime Definitions, specifications and
conformity criteria ECHA Candidate List
Candidate List of substances of very high concern for
EN 680 Authorisation(published in accordance with Article 59(10) of the
EN 680:2005, Determination of the drying shrinkage of REACH Regulation), https://echa.europa.eu/candidate-list-
autoclaved aerated concrete table, version 17.01.2023
EN 772-1 REGULATION (EU) No 528/2012
EN 772-1:2011+A1:2015, Methods of test for masonry units - REGULATION (EU) No 528/2012 OF THE EUROPEAN
Part 1: Determination of compressive strength PARLIAMENT AND OF THE COUNCIL
of 22 May 2012 concerning the making available on the market
EN 772-13 and use of biocidal products
EN 772-13:2000, Methods of test for
masonry units - Part 13: Determination of net and gross dry Further References
density of masonry units (except for natural stone)
IBU 2021
EN 1745 Institut Bauen und Umwelt e.V.: General
EN 1745:2020, Masonry and masonry products. Methods for Instructions for the EPD programme of Institut Bauen und
determining thermal properties Umwelt e.V., Version 2.0, Berlin: Institut Bauen und Umwelt
e.V., 2021
EN 15804 www.ibu-epd.com
EN 15804:2012+A2:2019+AC:2021, Sustainability of
construction works — Environmental Product Declarations — O. Kreft, C. Fudge, P. Walczak, 2022
Core rules for the product category of construction products. O. Kreft, C. Fudge, P. Walczak, 2022. Roadmap für eine
treibhausgasneutrale
ISO 14025 Porenbetonindustrie in Europa, Mauerwerk, Volume 26, Issue
EN ISO 14025:2011, Environmental labels and declarations — 2, Pages 77-84. https://doi.org/10.1002/dama.202200004
Type III environmental declarations — Principles and
procedures. P. Walczak
P. Walczak, AAC Life Cycle: how long can
PN-H-97021 autoclaved aerated concrete buildings be used, 7th ICAAC,
PN-H-97021:1998, polish version, Aluminium -- Proszek Prague, DOI: 10.1002/cepa.2095
płatkowy do produkcji betonu komórkowego
6 Environmental Product Declaration - Solbet Sp. z o.o. - Autoclaved Aerated Concreate (AAC)
PCR Part A
PCR - Part A: Calculation rules for the Additional Documents
Life Cycle Assessment and Requirements on the Background
Report, version 1.3, Institut Bauen und Umwelt e.V., 2021. P. Walczak, SOLBET Research Center Department, 2022
P. Walczak, SOLBET Research Center Department, 2022.
PCR Part B Report of Autoclaved Aerated Concrete Carbonation, Research
PCR – Part B: PCR – Part B: Requirements on the EPD for Center Department - SOLBET, Solec Kujawski, Poland.
Aerated Concrete, v1., Institut Bauen und Umwelt e.V.,
www.bau-umwelt.com, 2023 DoP of AAC are available on the websites:
Sphera LCA FE (GaBi ts) www.solbet.pl
GaBi ts dataset documentation for the software-system and www.solbet-lubartow.pl
databases, LBP, University of Stuttgart and thinkstep, www.solbet-kolbuszowa.com.pl
Leinfelden-Echterdingen, 2023 (https://www.gabi- www.solbet-stw.pl
software.com/support/gabi).
7 Environmental Product Declaration - Solbet Sp. z o.o. - Autoclaved Aerated Concreate (AAC)
Publisher
Institut Bauen und Umwelt e.V. +49 (0)30 3087748- 0
Hegelplatz 1 info@ibu-epd.com
10117 Berlin www.ibu-epd.com
Germany
Programme holder
Institut Bauen und Umwelt e.V. +49 (0)30 3087748- 0
Hegelplatz 1 info@ibu-epd.com
10117 Berlin www.ibu-epd.com
Germany
Author of the Life Cycle Assessment
Sphera Solutions GmbH +49 711 341817-0
Hauptstraße 111- 113 info@sphera.com
70771 Leinfelden-Echterdingen www.sphera.com
Germany
Owner of the Declaration
SOLBET SP. Z O.O. +48 52 387 41 00
Torunska 71 sekretariat@solbet.pl
86-050 Solec Kujawski www.solbet.pl
Poland
8 Environmental Product Declaration - Solbet Sp. z o.o. - Autoclaved Aerated Concreate (AAC)
