ENVIRONMENTAL PRODUCT DECLARATION
as per ISO 14025 and EN 15804+A1
Owner of the Declaration Kaimann GmbH
Programme holder Institut Bauen und Umwelt e.V. (IBU)
Publisher Institut Bauen und Umwelt e.V. (IBU)
Declaration number EPD-KAI-20200015-IBC1-EN
Issue date 08.06.2020
Valid to 07.06.2025
Kaiflex EPDMplus
Kaimann GmbH
www.ibu-epd.com | https://epd-online.com
Umwelt Produktdeklaration Name des Herstellers – Name des Produkts
1. General Information
Kaimann GmbH Kaiflex EPDMplus
Programme holder Owner of the declaration
IBU – Institut Bauen und Umwelt e.V. Kaimann GmbH
Panoramastr. 1 Hansastraße 2-5
10178 Berlin 33161 Hövelhof
Germany
Declaration number Declared product / declared unit
EPD-KAI-20200015-IBC1-EN 1 m3 insulation material Kaiflex EPDMplus
This declaration is based on the product Scope:
category rules: Product line Kaiflex EPDMplus
Insulating materials made of foam plastics, 06.2017 Thermal insulation material made of flexible
(PCR checked and approved by the SVR) elastomeric foam for technical building equipment and
industrial installations.
Issue date The EPD is performed in agreement with the demands
08.06.2020 of PCR Part A with reference to EN 15804+A1:2013
and PCR Part B: Requirements on the EPD for
insulating materials made of foam plastics.
Valid to
The EPD is based on the average Kaiflex EPDMplus
07.06.2025
production from two different variations produced in
one plant in Germany.
The owner of the declaration shall be liable for the
underlying information and evidence; the IBU shall not
be liable with respect to manufacturer information, life
cycle assessment data and evidences.
The EPD was created according to the specifications
of EN 15804+A1. In the following, the standard will be
simplified as EN 15804.
Verification
The standard EN 15804 serves as the core PCR
Independent verification of the declaration and data
according to ISO 14025:2010
Dipl. Ing. Hans Peters internally x externally
(chairman of Institut Bauen und Umwelt e.V.)
Dr. Alexander Röder Matthias Klingler
(Managing Director Institut Bauen und Umwelt e.V.)) (Independent verifier appointed by SVR)
2. Product
2.1 Product description/Product definition For the application and use the respective national
Kaiflex EPDMplus is a flexible closed cell rubber provisions apply.
insulation that prevents condensation and reduces
energy loss. By incorporating a water vapour barrier
into the insulation cell structure Kaiflex EPDMplus can 2.2 Application
eliminate water vapour migration and retain its Kaiflex EPDMplus is available in tube and sheets for
performance over the entire system life. This EPD use on air-conditioning, refrigeration, chilled water,
covers the Kaiflex EPDMplus product family including heating and hot water pipes and air-distribution
Kaiflex EPDMplus tubes and sheets. ductwork. In addition to preventing condensation and
saving energy, Kaiflex EPDMplus also performs an
For the placing on the market of the product in the acoustic function, absorbing sound and dampening
European Union/European Free Trade Association duct wall vibration. With inherent anti-microbial
(EU/EFTA) (with the exception of Switzerland) resistance as standard, and a Class D fire rated,
Regulation (EU) No. 305/2011 (CPR) applies. The closed cell rubber that is completely dust and fibre
product needs a declaration of performance taking into free, Kaiflex EPDMplus can be used in any kind of
consideration EN 14304:2009 Thermal insulation public, commercial or industrial building without
products for building equipment and industrial impacting on health or the quality of air. Outdoor
installations - Factory made flexible elastomeric foam application requires protection against UV-radiation.
(FEF) products - Specification, and the CE-marking.
2 Environmental Product Declaration Kaimann GmbH – Kaiflex EPDMplus
2.3 Technical Data which are not on the candidate list, exceeding 0.1
percentage by mass: no.
3) Biocide products were added to this construction
Constructional data product or it has been treated with biocide products
Name Value Unit (this then concerns a treated product as defined by the
Gross density 84 kg/m3 (EU) Ordinance on Biocide Products No. 528/2012):
Water vapour diffusion resistance no.
µ ≥ 4500 -
factor acc. to EN 12088
λϑ = 0.038 2.6 Manufacture
+ 8.0 · Manufacturing happens in a single plant in Germany.
Thermal conductivity W/(mK)
10E-5 ϑ + Upon delivery, the raw materials are either stored in a
7*10E-7*ϑ² warehouse or used in the production shortly after. The
Thermal conductivity at -10 °C 0.037 W/(mK) first step in the production of Kaiflex EPDMplus is to
Thermal conductivity at 0 °C 0.038 W/(mK) mix the raw materials in a kneader and to roll-out the
Thermal conductivity at 10 °C 0.039 W/(mK) resulting mixture which is then cut into sheets. The flat
Performance data of the product in accordance with sheets are passed through an industrial cooler and
the declaration of performance with respect to its cooled-off. The cooled-off sheets are granulated and
essential characteristics according to EN 14304:2009 the granulates are temporarily stored at room
Thermal insulation products for building equipment and temperature before entering the compounding plant.
industrial installations - Factory made flexible
elastomeric foam (FEF) products - Specification. In a next step, the different types of granulates enter
the compounding plant for mixing. The resulting
elastomer compound is pushed through one of five
extruders and carried on a conveyer belt through an
2.4 Delivery status industrial furnace for foaming. After foaming, the
The EPD is declared as an average product of one endless sheets are passed through an industrial cooler
plant of one manufacturer. It looks at the average upon which a continuous longitudinal cut is applied to
environmental performance of six product varieties cut sheets into the right width. If applicable, adhesive
from the product line Kaiflex EPDMplus. This is in coating is applied on one side of the sheets. Finally, a
accordance with the classification rules for group 1c) traverse cut trims the continuous sheet into sheets of
from PCR Part A paragraph 5.2. The products are: various sizes.
2.7 Environment and health during
 Kaiflex EPDMplus tube
manufacturing
 Kaiflex EPDMplus sheet
The manufacturer of the product complies with national
manufacturing guidelines and regulations such as the
Sheets are available from d = 3 mm to 32 mm. Tubes German Energy Saving Regulation (EnEV) and the
N
are available from d = 10 mm to 32 mm German Renewable Energy Act (EEG). In addition,
N
KAIMANN’s environmental management system is
2.5 Base materials/Ancillary materials certified in accordance with ISO 9001/14001/50001.
Kaiflex EPDMplus is based on synthetic rubber and
consists of several components. The following table 2.8 Product processing/Installation
shows the components clustered into substance The installation of Kaiflex EPDMplus requires basic
groups: tools such as cutters and scissors. No additional
specific protection, beyond normal protective clothes,
 Rubber and polymers: 19% is required. Liquid oxygen can react explosively in
conjunction with organic material such as Kaiflex
 Fillers and pigments: 5%
EPDMplus insulation material. To avoid the diffusion of
 Blowing agent: 8.5%
oxygen, a complete seal must be affected. Butt joints
 Vulcanisation system, additives, plasticizer: and overlapping areas must also be made airtight
15.5% using Kaiflex adhesive.
 Flame retardant: 48%
2.9 Packaging
 Stabilizer: 4%
Kaiflex EPDMplus is packaged in cardboard boxes,
polyethylene film, and polypropylene bags, both in
Rubber and polymer are the base material. Fillers and varying sizes. Cardboard boxes and polypropylene
pigments are for firmness and colour. The blowing bags are placed on wooden EURO pallets.
agent causes the volume increase and expansion
process during the manufacture of the product. The
vulcanisation system, additives, and plasticizer sure 2.10 Condition of use
flexibility and workability. The flame retardants ensure Changes in materials composition of the product
the fire resistance of the end-product, and the during the use-phase only occur in case of
adhesives and stabilizers are for processing and extraordinary effects.
process control.
2.11 Environment and health during use
1) This product/article/at least one partial article An odour should be considered normal. The odour will
contains substances listed in the candidate list dissipate during use (about 4 weeks) because the cells
(16.01.2020) exceeding 0.1 percentage by mass: no. are exchanged with the air.
2) This product/article/at least one partial article
contains other CMR substances in categories 1A or 1B
3 Environmental Product Declaration Kaimann GmbH – Kaiflex EPDMplus
moisture ingress and requires no additional water
2.12 Reference service life vapour barrier.
Mechanical destruction
Since the use stage (B1-B7) is not fully declared, the Kaiflex insulation materials are flexible foams and
declaration of the reference service life is only display limited mechanical rigidity. If the material
voluntary. should be subjected to mechanical loads, it should be
protected accordingly.
2.13 Extraordinary effects
2.14 Re-use phase
Fire At the end-of-life, the product can be used for energy
recovery in a waste incineration plant, as well as the
plastic from packaging. The cardboard and wooden
Fire protection pallets from packaging can be recycled.
Name Value
Building material class E (sheets) / EL (tubes) 2.15 Disposal
Burning droplets - The product is disposed of in accordance with local
Smoke gas development - regulations governed by the European Waste
Catalogue (waste code: 07 wastes from organic
Water chemical processes - 07 02 13 waste plastic).
Formed from thousands of independently water-
resistant cells, Kaiflex insulation is naturally resistant to 2.16 Further information
Additional information about the product is available on
https://kaimann.com/.
3. LCA: Calculation rules
3.1 Declared Unit as well as buildings to manufacture the declared unit
The declared unit is 1 m³ of the thermal insulation are neglected. On average, 0.49 kWh electricity and
material for technical building equipment and industrial 2.65 kWh natural gas are required for the
installations Kaiflex EPDMplus including packaging manufacturing of 1m³ Kaiflex EPDMplus. This data
materials. The declared unit refers to the product as it was provided by Kaimann GmbH. This module also
leaves the factory gate. The gross density is the includes packaging with plastics and cardboard and
average density of al declared products, weighted by wooden pallets. The biogenic carbon stored is
production volume. declared in the result section.
Declared unit Module A4: The transport of Kaiflex EPDMplus from
Name Value Unit the factory gate to the site of assembly is represented
Gross density 84 kg/m3 through generic background data. The transportation
Conversion factor to 1 kg 84 - distances are based on average transportation data
Declared unit 1 m3 provided by the manufacturer.
Module A5: The assembly can be done manually
without the use of any electrical equipment. Only glue
3.2 System boundary (Kaiflex Special glue) is required for the assembly of
The type of EPD is cradle to gate with options. The Kaiflex EPDMplus. Packaging material from module A3
system boundaries of the EPD follow the modular is disposed of here: Plastic packaging is incinerated,
structure of EN 15804 (according to EN 15804, section and cardboard and the wooden pallet are re-used.
6.2.1). Only the declaration of the product stage
modules A1 to A3 is mandatory for compliance with Modules B1-B7: No resource use and impacts occur
EN15804. The declaration of the modules of other life during the use phase of the products.
cycle stages is optional. Resources from the
ecosphere and technosphere enter the system on Modules C1&C3: Dismantling of Kaiflex EPDMplus is
stage A1 and leave the system on stage C4. The done manually without using any electrical equipment.
following life cycle stages are considered: No processing is required before disposal. Therefore,
module C1 and C3 are disregarded.
Module A1: The system boundaries comprise raw
material extraction and supply from cradle to factory Module C2: The products to be disposed of are
gate and is represented through generic background transported to the waste treatment facility.
data sets.
Module C4: The waste is treated according to the
Module A2: The transport of the raw materials from waste framework directive of the European Union.
the factory gate to the point of manufacturing is
represented through generic background data sets. Module D: Potential impacts and benefits from energy
The transportation distances have been provided by recovery and recycling are described.
the manufacturer.
3.3 Estimates and assumptions
Module A3: The manufacturing includes Module A2: Raw materials are transported to the
manufacturer-specific material and energy data which manufacturer by road transport and shipping.
are represented through generic data sets. Machinery Information on the transportation distances was
4 Environmental Product Declaration Kaimann GmbH – Kaiflex EPDMplus
provided by the manufacturer. For the calculation, the available. Datasets from the GaBi database are
distances were weighted by the mass of the respective assumed to have a high quality.
raw materials. There are no materials or processes that are left out
because they are under the cut-off threshold.
Module A3: No production waste is assumed during
the production of Kaiflex. 3.7 Period under review
The production data refers to the average of the year
Module A4: Kaiflex EPDMplus is distributed in Europe. 2018.
The average transportation distance per declared unit
was calculated based on the sales volume and 3.8 Allocation
average transportation distance per country where No allocation is carried out.
Kaiflex EPDMplus is distributed. Based on the sum
product of sales volume multiplied with road 3.9 Comparability
transportation, the total transportation distances were Basically, a comparison or an evaluation of EPD data
calculated and divided by the total sales volume to is only possible if all the data sets to be compared
calculate the average transportation distance per were created according to EN 15804 and the building
declared unit. As a result, the average road context, respectively the product-specific
transportation distance per declared unit is 743 km, characteristics of performance, are taken into account.
and the average ship transportation distance is 97 km.
No loss during transportation is assumed. As a background database GaBi database
professional database (version from September 2019)
Module A5: Kaiflex EPDMplus is assembled by by thinkstep AG was used and has been
manual labour under use of adhesives. It is assumed complemented by data sets from GaBi extension
that no further energy or materials are required in this databases as well as data sets from the EuGeos
module, and that consumers of Kaiflex EPDMplus database 15804-IA database version 2.1 by EuGeos
order correct product sizes and thus avoid waste Ltd.
production during the assembly. The packaging
materials are disposed of by re-using (cardboard and
wooden pallet) and by incineration (polyethylene and
polypropylene).
Module C2: The average distance of the
disassembled product to the point of disposal is
assumed to be 75 kilometres covered by road.
Module C4: The product is incinerated.
3.4 Cut-off criteria
All material flows in module A1 are covered and almost
all material and energy flows in module A3 are
covered. Neglected material or energy flows have a
mass or energy contribution of less than one percent
per process and contribute to less than 5% of mass
and energy flows of a module. Infrastructure such as
office buildings and the manufacturing hall as well as
the machinery required to produce the product have
not been considered.
3.5 Background data
The LCA model underlying this EPD was created in
openLCA 1.10 developed by GreenDelta GmbH. As a
background database GaBi database professional
database (version from September 2019) by thinkstep
AG was used and has been complemented by data
sets from GaBi database extension databases as well
as data sets from the EuGeos database 15804-IA
database version 2.1 by EuGeos Ltd.
3.6 Data quality
The life cycle inventory for the assessed product is
based on an internal assessment of manufacturing and
environmental data, assessment of LCA-relevant data
for the supply chain and energy measurement within
the factors. The required product flows for creation of
the product system were handed over to GreenDelta
GmbH.
All data was scrutinised and found to be plausible and
consistent and were therefore found to be
representative.
Some of the background data sets are more than 10
years old but were used when no recent dataset was
5 Environmental Product Declaration Kaimann GmbH – Kaiflex EPDMplus
.
4. LCA: Scenarios and additional technical information
The following technical scenario information serves as
a basis for the declared modules. All values refer to the
declared unit of 1 m³.
Transport to the building site (A4)
Name Value Unit
Transport distance (road) 518 km
transport distance (ship) 31 km
Installation into the building (A5)
Name Value Unit
Auxiliary 1.6 kg
Water consumption 0 m3
Other resources 0 kg
Electricity consumption 0 kWh
Other energy carriers 0 MJ
Material loss 0 kg
Output substances following waste
16.5 kg
treatment on site
Dust in the air 0 kg
VOC in the air 0 kg
The 16.5 kg are the sum of all packaging materials per
declared unit.
End of life (C1-C4)
Name Value Unit
Collected separately 85.6 kg
Collected as mixed construction
0 kg
waste
Reuse 0 kg
Recycling 0 kg
Energy recovery 85.6 kg
Landfilling 0 kg
84 kg Kaiflex and 1.6 kg special glue are incinerated
for energy recovery.
Reuse, recovery and/or recycling potentials (D),
relevant scenario information
Module D includes the credits of the incineration
processes from modules C4 and A5 (packaging waste)
at a waste incineration plant with an assumed
efficiency of R1<0.6.
6 Environmental Product Declaration Kaimann GmbH – Kaiflex EPDMplus
5. LCA: Results
The life cycle impact assessment method is based on EN15804. Energy indicators for resource use utilise the
lower calorific value.
DESCRIPTION OF THE SYSTEM BOUNDARY (X = INCLUDED IN LCA; MND = MODULE NOT DECLARED;
MNR = MODULE NOT RELEVANT)
BENEFITS AND
CONSTRUCTI LOADS
PRODUCT STAGE ON PROCESS USE STAGE END OF LIFE STAGE BEYOND THE
STAGE SYSTEM
BOUNDARIES
7 Environmental Product Declaration Kaimann GmbH – Kaiflex EPDMplus
lairetam
waR
ylppus tropsnarT
gnirutcafunaM
eht
morf
tropsnarT
etis
eht
ot
etag
ylbmessA esU
ecnanetniaM
riapeR
tnemecalpeR tnemhsibrufeR
ygrene
lanoitarepO esu
retaw
lanoitarepO esu
noitcurtsnoc-eD
noitilomed tropsnarT
gnissecorp
etsaW
lasopsiD -esueR -yrevoceR -gnilcyceR laitnetop
A1 A2 A3 A4 A5 B1 B2 B3 B4 B5 B6 B7 C1 C2 C3 C4 D
X X X X X MND MND MNR MNR MNR MND MND MND X MND X X
RESULTS OF THE LCA - ENVIRONMENTAL IMPACT according to EN 15804+A1: 1 m³
Parameter Unit A1 A2 A3 A4 A5 C2 C4 D
GWP [kg CO2-Eq.] 2.07E+2 9.30E+0 2.64E+1 7.14E+0 1.27E+1 1.05E+0 1.96E+2 -2.20E+2
ODP [kg CFC11-Eq.] 5.12E-5 9.90E-7 2.23E-7 1.33E-6 2.04E-7 1.96E-7 1.35E-13 -2.23E-7
AP [kg SO2-Eq.] 1.27E+0 1.35E-1 8.69E-2 2.91E-2 1.36E-2 4.14E-3 2.29E-2 -2.14E-1
EP [kg (PO4)3--Eq.] 7.57E-1 1.71E-2 2.05E-2 6.73E-3 5.93E-3 9.77E-4 5.24E-3 -5.14E-2
POCP [kg ethene-Eq.] 5.58E-2 4.05E-3 5.07E-3 1.20E-3 1.79E-3 1.73E-4 1.33E-3 -1.09E-2
ADPE [kg Sb-Eq.] 3.68E-3 1.60E-5 9.33E-6 2.13E-5 8.88E-6 3.15E-6 1.32E-6 -1.30E-5
ADPF [MJ] 4.32E+3 1.31E+2 3.19E+2 1.10E+2 1.06E+2 1.62E+1 8.29E+1 -1.70E+3
GWP = Global warming potential; ODP = Depletion potential of the stratospheric ozone layer; AP = Acidification potential of land and water; EP =
Caption Eutrophication potential; POCP = Formation potential of tropospheric ozone photochemical oxidants; ADPE = Abiotic depletion potential for non-
fossil resources; ADPF = Abiotic depletion potential for fossil resources
RESULTS OF THE LCA - RESOURCE USE according to EN 15804+A1: 1 m³
Parameter Unit A1 A2 A3 A4 A5 C2 C4 D
PERE [MJ] 2.59E+2 1.04E+0 2.79E+2 1.19E+0 7.80E+0 1.75E-1 2.30E+1 -5.28E+2
PERM [MJ] 1.01E+1 0.00E+0 2.35E+2 0.00E+0 0.00E+0 0.00E+0 0.00E+0 -2.35E+2
PERT [MJ] 2.69E+2 1.04E+0 5.13E+2 1.19E+0 7.80E+0 1.75E-1 2.30E+1 -7.63E+2
PENRE [MJ] 1.30E+3 1.32E+2 2.24E+2 1.12E+2 2.24E+2 1.64E+1 3.41E+3 -1.70E+3
PENRM [MJ] 3.33E+3 0.00E+0 1.16E+2 0.00E+0 -1.16E+2 0.00E+0 -3.33E+3 0.00E+0
PENRT [MJ] 4.62E+3 1.32E+2 3.40E+2 1.12E+2 1.08E+2 1.64E+1 8.29E+1 -1.70E+3
SM [kg] 0.00E+0 0.00E+0 0.00E+0 0.00E+0 0.00E+0 0.00E+0 0.00E+0 0.00E+0
RSF [MJ] 0.00E+0 0.00E+0 0.00E+0 0.00E+0 0.00E+0 0.00E+0 0.00E+0 0.00E+0
NRSF [MJ] 0.00E+0 0.00E+0 0.00E+0 0.00E+0 0.00E+0 0.00E+0 0.00E+0 0.00E+0
FW [m³] 6.91E+0 1.64E-2 7.24E-1 1.88E-2 1.05E-1 2.77E-3 6.38E-1 -3.89E+0
PERE = Use of renewable primary energy excluding renewable primary energy resources used as raw materials; PERM = Use of
renewable primary energy resources used as raw materials; PERT = Total use of renewable primary energy resources; PENRE = Use of
non-renewable primary energy excluding non-renewable primary energy resources used as raw materials; PENRM = Use of non-
Caption
renewable primary energy resources used as raw materials; PENRT = Total use of non-renewable primary energy resources; SM = Use
of secondary material; RSF = Use of renewable secondary fuels; NRSF = Use of non-renewable secondary fuels; FW = Use of net fresh
water
RESULTS OF THE LCA – OUTPUT FLOWS AND WASTE CATEGORIES according to EN 15804+A1:
1 m³
Parameter Unit A1 A2 A3 A4 A5 C2 C4 D
HWD [kg] 3.05E-2 5.21E-9 9.50E-3 4.88E-11 5.23E-8 0.00E+0 5.33E-7 -1.71E-3
NHWD [kg] 7.86E+1 1.02E-1 9.01E+0 9.55E-4 5.67E+0 0.00E+0 6.61E+1 -3.18E+2
RWD [kg] 1.63E-2 5.83E-5 2.79E-3 5.46E-7 1.01E-3 0.00E+0 3.91E-3 -4.88E-3
CRU [kg] 0.00E+0 0.00E+0 0.00E+0 0.00E+0 1.37E+1 0.00E+0 0.00E+0 0.00E+0
MFR [kg] 0.00E+0 0.00E+0 0.00E+0 0.00E+0 0.00E+0 0.00E+0 0.00E+0 0.00E+0
MER [kg] 0.00E+0 0.00E+0 0.00E+0 0.00E+0 0.00E+0 0.00E+0 0.00E+0 0.00E+0
EEE [MJ] 0.00E+0 0.00E+0 0.00E+0 0.00E+0 0.00E+0 0.00E+0 0.00E+0 0.00E+0
EET [MJ] 0.00E+0 0.00E+0 0.00E+0 0.00E+0 6.94E+1 0.00E+0 2.00E+3 0.00E+0
HWD = Hazardous waste disposed; NHWD = Non-hazardous waste disposed; RWD = Radioactive waste disposed; CRU = Components
Caption for re-use; MFR = Materials for recycling; MER = Materials for energy recovery; EEE = Exported electrical energy; EEE = Exported
thermal energy
Additional Technical scenario:
Biogenic carbon is not included in the results. It enters the product system with wood and cardboard in modules
A3 and is ‘released’ by being an avoided burden in module A5 (declared in module D) and has thus no net-effect
on the overall results. The wooden pallet has approximately 23 kg biogenic CO2, and the carboard has 16 kg.
6. LCA: Interpretation
Environmental Impacts
The production of the blowing agent uses the most
fresh water.
Most environmental impact categories are dominated
by module A1 raw material supply. The production of Hazardous waste disposed (HWD)
the blowing agent is the largest contributors. For the Most of the hazardous waste comes from the
global warming potential, the incineration of the production of the blowing agent in A1 and the
product in module C4 is another major source of production of the plastic packaging in A3.
greenhouse gas emissions.
Non-hazardous waste disposed (NHWD)
Renewable primary energy as energy carrier This impact category is dominated by module A1 raw
(PERE) material supply and the incineration residues in module
Renewable energy is used in the production of the raw C4.
materials and in the production of the packaging The main contributor is the production of the flame
(mainly the wooden pallet). Likewise, energy is retardant.
released in the incineration process (D).
Radioactive waste disposed (RWD)
Renewable primary energy resources as material This impact category is dominated by module A1 raw
utilization (PERM) material supply.
The wood of the pallet acts as a storage for renewable Most radioactive waste stems from the production of
energy. By re-using the pallet, the same amount of the flame retardant.
energy is credited in module D.
Conclusion
Use of net fresh water (FW) The production of the blowing agent is the largest
This impact category is dominated by module A1 raw contributor to the environmental impacts of EPDMplus.
material supply.
7. Requisite evidence
VOC without NIK <5 μg/m3
7.1 VOC emissions Carcinogenic Substances <1 μg/m3
The Volatile Organic Compound (VOC) emissions
have been tested by Eurofins Product Testing A/S by AgBB overview of results (3 days [µg/m³])
using the Committee for health-related evaluation of Name Value Unit
building products/Deutsches Institut für Bautechnik TVOC (C6 - C16) <5 μg/m3
(AgBB/DIBt) test method in 09.2013. Sum SVOC (C16 - C22) <5 μg/m3
R (dimensionless) <1 -
AgBB overview of results (28 days [µg/m³]) VOC without NIK <5 μg/m3
Name Value Unit Carcinogenic Substances <1 μg/m3
TVOC (C6 - C16) <5 μg/m3
7.2 Leaching performance
Sum SVOC (C16 - C22) <5 μg/m3
The concentration of water-soluble chloride ions is 300
R (dimensionless) <1 -
mg/kg according to EN 13468:2001.
8 Environmental Product Declaration Kaimann GmbH – Kaiflex EPDMplus
8. References
AGBB/DIBt Sustainability Software, Data, and Consulting
Deusches Institut für Bautechnik 2018: Anforderungen
an die Innenraumluftqualität in Gebäuden: ISO 9001
Gesundheitliche Bewertung der Emissionen von ISO 9001:2015, Quality management systems -
flüchtigen organischen Verbindungen (VVOC, VOC Requirements
und SVOC) aus Bauprodukten
ISO 14001
EN 12088 ISO 14001:2015-0/, Environmental management
EN 12088:2013, Thermal insulating products for systems - Requirements with guidance for use
building applications. Determination of long term water
absorption by diffusion ISO 50001
ISO 50001:2018-08, Energy management systems -
EN 13468 Requirements with guidance for use
EN 13468:2001, Thermal insulating products for
building equipment and industrial installations - openLCA 1.10
Determination of trace quantities of water soluble open LCA 1.10.2 (2020), Sustainability Software,
chloride, fluoride, silicate, and sodium ions and pH Databases, and Consulting. Developed by GreenDelta
GmbH. http://www.openlca.org/
EN 14304
EN 14304:2009+A1:2013, Thermal insulation products PCR Part A
for building equipment and industrial installations - PCR Part A Version 1.8, Calculation Rules for the Life
Factory made flexible elastomeric foam (FEF) Cycle Assessment and Requirements on the Project
products - Specification Report
EN 15804 PCR Part B
EN 15804:2012+A1:2013, Nachhaltigkeit von PCR Part B Version 1.6, Requirements on the EPD for
Bauwerken – Umweltproduktdeklarationen – insulating materials made of foam plastics
Grundregeln für die Produktkategorie Bauprodukte
REACH 2006
EuGeos database REGULATION (EC) No 1907/2006 OF THE
LCA database by EuGeos Limited EUROPEAN PARLIAMENT AND OF THE COUNCIL
concerning the Registration, Evaluation, Authorisation
Eurofins and Restriction of Chemicals (REACH)
Eurofins Product Testing A/S, Galten, Denmark
SVHC 2019
European waste catalogue 2014 Candidate List of substances of very high concern for
COMMISSION DECISION amending Decision Authorisation (SVHC), European Chemicals Agency,
2000/532/EC on the list of waste pursuant to Directive Helsinki, Finland
2008/98/EC of the European Parliament and of the
Council thinkstep AG
Sustainability Software, Data, and Consulting
GABI database
LCA database SP 39. thinkstep AG. Echterdingen
2019
GreenDelta GmbH
9 Environmental Product Declaration Kaimann GmbH – Kaiflex EPDMplus
Publisher
Institut Bauen und Umwelt e.V. Tel +49 (0)30 3087748- 0
Panoramastr. 1 Fax +49 (0)30 3087748- 29
10178 Berlin Mail info@ibu-epd.com
Germany Web www.ibu-epd.com
Programme holder
Institut Bauen und Umwelt e.V. Tel +49 (0)30 - 3087748- 0
Panoramastr 1 Fax +49 (0)30 – 3087748 - 29
10178 Berlin Mail info@ibu-epd.com
Germany Web www.ibu-epd.com
Author of the Life Cycle
Assessment Tel +49 30 6292 4320
GreenDelta GmbH Fax -
Kaiserdamm 13 Mail gd@greendelta.com
14057 Berlin Web https://www.greendelta.com
Germany
Owner of the Declaration
Kaimann GmbH Tel +49 5257 98 50 - 0
Hansastraße 2-5 Fax +49 5257 98 50 590
33161 Hövelhof Mail info@kaimann.de
Germany Web https://www.kaimann.com
