ENVIRONMENTAL PRODUCT DECLARATION
as per ISO 14025 and EN 15804+A1
Owner of the Declaration NedZink B.V.
Programme holder Institut Bauen und Umwelt e.V. (IBU)
Publisher Institut Bauen und Umwelt e.V. (IBU)
Declaration number EPD-NED-20200255-IBC1-EN
Issue date 15.06.2021
Valid to 14.06.2026
NedZink NATUREL
NedZink B.V.
www.ibu-epd.com | https://epd-online.com
Umwelt Produktdeklaration Name des Herstellers – Name des Produkts
1. General Information
NedZink B.V. NedZink NATUREL
Programme holder Owner of the declaration
IBU – Institut Bauen und Umwelt e.V. NedZink B.V.
Panoramastr. 1 Hoofdstraat 1
10178 Berlin 6024 AA, Budel-Dorplein
Germany Netherlands
Declaration number Declared product / declared unit
EPD-NED-20200255-IBC1-EN 1kg NedZink® NATUREL, bright-rolled titanium zinc
This declaration is based on the product Scope:
category rules: The Life Cycle Assessment (LCA) was carried out
Building metals, 11.2017 according to ISO 14040, ISO 14044 and EN 15804.
(PCR checked and approved by the SVR) The LCA is performed for NedZink® NATUREL
manufactured by NedZink B.V. in Budel-Dorplein,
Netherlands.
Issue date
The natural rolled zinc from NedZink covered by this
15.06.2021
EPD can be used in buildings as roof, façade or
rainwater systems.
Valid to The LCA was carried out for the manufacturing phase
14.06.2026 of the declared product, containing information on raw
and secondary material production, transport and
packaging (cradle to gate). Possible credits after the
end of life phase (module D), waste disposal (C4) and
transport to waste disposal (C2) are also included.
The owner of the declaration shall be liable for the
underlying information and evidence; the IBU shall not
be liable with respect to manufacturer information, life
cycle assessment data and evidences.
The EPD was created according to the specifications
of EN 15804+A1. In the following, the standard will be
simplified as EN 15804.
Verification
The standard EN 15804 serves as the core PCR
Independent verification of the declaration and data
according to ISO 14025:2010
Dipl. Ing. Hans Peters internally x externally
(chairman of Institut Bauen und Umwelt e.V.)
Dr. Alexander Röder Mr Olivier Muller
(Managing Director Institut Bauen und Umwelt e.V.)) (Independent verifier)
2. Product
2.1 Product description/Product definition
NedZink® NATUREL is titanium zinc produced by For the placing on the market of the product in the
NedZink according to EN 988. European Union/European Free Trade Association
Small quantities, as specified in EN 988, of the alloy (EU/EFTA) (with the exception of Switzerland)
elements copper, titanium and aluminium are added to Regulation (EU) No. 305/2011 (CPR) applies. The
electrolytically refined zinc (with a purity of min. product needs a Declaration of Performance taking
99,995% Zn, Z1 according to EN 1179). into consideration EN 14782:2006, Self-supporting
The chemical composition, mechanical and physical metal sheet for roofing, external cladding and internal
properties and measurement tolerances are lining, or EN 14783:2013, Fully supported metal sheet
determined in the KOMO product certificate and and strip for roofing, external cladding and internal
certified as NedZink NTZ® by Lloyd's Register Product lining, and the CE-marking.
certificate (approval No QIS 122). For the application and use the respective national
The defined material properties are checked by an provisions apply.
independent and neutral research institute. This
product certification and the ISO 9001 certificate for
the quality management system at NedZink assure a
constant and uniform high quality standard.
2 Environmental Product Declaration NedZink B.V. – NedZink Naturel
2.2 Application product does not contain substances with carcinogenic
NedZink® NATUREL titanium zinc coils, sheets, strips mutagenic reprotoxic (CMR) properties >0.1%.
and profiles are used for:
- roof and façade cladding (CE-marked based on 2.6 Manufacture
EN14782:2006, Self-supporting metal sheet for The manufacturing process of high grade rolled zinc
roofing, external cladding and internal lining or includes the following steps:
EN14783:2013, Fully supported metal sheet and strip
for roofing, external cladding and internal lining) Pre-alloy:
- interior use In order to improve the properties of zinc, and for
- roof drainage systems (gutters, downpipes and energy saving purposes, a pre-alloy with titanium,
accessories according to EN612) copper and aluminium is prepared in an induction
- ornaments furnace. This pre-alloy is poured into ingots.
2.3 Technical Data Melting:
The main constructional data are presented in the In the melting furnace the Special High Grade (SHG)
following table: zinc and the ingots are mixed homogeneously. Zinc
with the right composition is pumped to the casting
Constructional data furnace.
Name Value Unit
Coefficient of thermal expansion 22 10-6K-1 Casting:
Tensile strength ≥ 150 N/mm2 Casting takes place from the casting furnace into a
Not vertical casting installation. The zinc is cast into blocks,
Compressive strength N/mm2
relevant cooled down with a closed water system and stored for
Modulus of elasticity ≥ 80000 N/mm2 further processing.
Melting point 420 °C
Thermal conductivity 110 W/(mK) Rolling and coiling:
Electrical conductivity at 20°C 17000000 Ω-1m-1 Blocks coming from the casting installation are
homogeneous pre-heated for the “hot rolling” process.
Density 7200 kg/m3
This takes place in a gas-fired continuous oven.
Required testing standards are described in EN 988.
During the hot rolling on a reversible rolling machine
the blocks are processed to a predefined thickness. At
Performance data of the product in accordance with
the end of the rolling installation the zinc is coiled and
the declaration of performance with respect to its
stored to cool off.
essential characteristics according to EN
On the reversible cold-rolling mill the coils are rolled to
14782 and EN 14783 respectively.
the desired final thickness. For cooling and lubrication
of the process a special emulsion is used
2.4 Delivery status
NedZink material is delivered in thicknesses from 0.5
Stretching and cutting:
to 1.5 mm. As average production data is considered,
Tension in the coils is released by a stretching-and
the LCIA results reflect the environmental profile of
straightening process. The zinc is uniquely marked and
weighted average product thickness: 0.727 mm.
slitted and cut to the desired width and length.
The maximum width of sheets, coils and strips is 1000
mm.
Quality control:
The standard sheets are delivered in 1000 x 2000 mm,
During the entire process extensive quality checks are
1000 x 2250 mm and 1000 x 3000 mm.
conducted by the manufacturer and Lloyd's Register.
Finished products are delivered to customer
Quality Management according to ISO 9001.
specification.
Product quality is checked by Lloyd's Register and
approved with an Industrial Quality Scheme Approval
Application rules:
Certificate QIS122.
EN988:1996, Zinc and zinc alloys - Specifications for
Additionally the quality control is audited by Kiwa and
rolled flat products for buildings
certified with KOMO product certificates:
EN612:2005, Eaves gutters with bead stiffened fronts
- BRL2034, K7054/04 zinc sheets
and rainwater pipes with seamed joints made of metal
- BRL2035, K7057/04 zinc gutters
sheet
- BRL2044, K7063/04 zinc downpipes
2.5 Base materials/Ancillary materials
2.7 Environment and health during
Components of NedZink alloy
manufacturing
The composition of bright rolled zinc from NedZink is in
The manufacturing process is carried out according to
accordance with EN988:
the rules as laid down in the environmental permit.
- Special-High-Grade zinc 99.995% (Z1 according to
NedZink’s policy follows the Total Quality Management
EN 1179)
(TQM). The directives of the Environmental
- Copper: 0.08 - 0.17%
Management System ISO14001 are an integral part of
- Titanium: 0.07 - 0.12%
the Quality Management System ISO9001.
- Aluminium: ≤ 0.015%
2.8 Product processing/Installation
Auxiliary substances
Basic principles:
Lubricant oil: 0.65 kg/t zinc.
NedZink material must be stored under dry and
ventilated conditions. This applies storage in
None of the components included in the final product is
warehouses, on building sites, on installation sites as
listed in the Candidate List of Substances of Very High
well as during transportation. Coils are to be stored on
Concern for Authorisation (SVHC) dated 01/2018. The
their original pallets.
3 Environmental Product Declaration NedZink B.V. – NedZink Naturel
Transportation should only be done in developing a natural protection layer of zinc
enclosed vehicles. carbonate.
Temperature deviations have to be avoided as it can In aquatic systems only a small part of the total zinc
result in varying humidity levels. concentration is available for organisms (bioavailable).
All contact between zinc and moisture (wet surface, It is related to the physical-chemical conditions of the
rain or dew) during handling and transportation must receiving water body.
be avoided. Wet surfaces (with or without protective
film) may not directly be covered. Health
When used according to their designated function,
The material is to be processed without tension. NedZink products will have no health effects.
Zinc is an essential metal, necessary for living
The thermal expansion has to be taken into account organisms. Zinc does not accumulate in the body.
when installing/handling the product. The recommended daily intake of zinc (in the correct
form) according to the WHO 15mg/day for men and
Mechanical deformation of zinc should be avoided in 12mg/day for women.
case the zinc temperature is not at least 7°C.
2.12 Reference service life
Further installation rules are listed on The service life depends on the correct application
www.nedzink.com. according to the guidelines for processing and
installation. The theoretical lifetime according to the
2.9 Packaging available literature is > 100 years.
The packaging material in use are wooden pallets, Service lifetime according to Bundesinstitut für Bau-
paper/cardboard and plastics (films and wires). All Stadt- und Raumforschung (BBSR): > 50 years.
packaging materials are reusable and/or recyclable, if
gathered separately. As the EPD scope is a cradle-to-gate with options, no
The take-back and recycling of our packaging in reference service life is declared in the LCA.
Germany is organized by Interseroh.
The standard ISO 15686 has not been considered.
2.10 Condition of use 2.13 Extraordinary effects
NedZink material develops a protective patina layer,
which darkens the material slightly over time due to a Fire
reaction with oxygen and carbon dioxide (air and The NedZink® products comply with EN13501-1: the
water). This layer is responsible for the high resistance requirements of building material Class A1 "non-
of titanium zinc against corrosion. combustible". (96/603/EC)
Zinc in contact with air creates a zinc-oxide. Due to the
influence of water a zinc-hydroxide is developed. In the Fire protection
final step a reaction with carbon dioxide creates a non- Name Value
water-soluble coating of basic zinc carbonate, being Building material class EN13501
A1
the patina. Therefore NedZink material does not DIN4102
require any maintenance and cleaning during the Burning droplets EN13501 D0
period of use. If the surface is slightly damaged, this Smoke gas development
-
naturally formed patina layer will heal itself. EN13501
NedZink material is UV-resistant, non-flammable and Smoke production
resistant to radiating heat. Direct contact with chemical Vaporization as zinc oxide (ZnO) occurs when heated
substances, especially those containing acids, has to above 650 °C. The produced ZnO smoke may cause
be avoided. A list of substances to be avoided can be zinc fever (diarrhoea, dry throat, feverish) when
found on www.nedzink.com. inhaled over some (period of) time. The effects
The material has a repellent effect to electrosmog disappear completely in 1 to 2 days after the
(electromagnetic radiation) and the effects of rain and inhalation.
snow may be neglected.
Water
2.11 Environment and health during use Zinc is not classified as hazardous for the aquatic
Environment environment.
The due to air and water formed patina (zinc
carbonate) is a natural protection layer. Due to this Mechanical destruction
patina the transfer of zinc ions via rain water is Given the metallic nature of the product, there will be
constantly reduced, because this protection layer is no environmental effect.
non-water-soluble.
Further transfer of zinc ions is mainly related to the air 2.14 Re-use phase
pollution with SO 2. Due to the reduction of SO 2 Disassembly:
concentration in the air, the zinc-concentration of During disassembly of a building construction or
precipitation in the rainwater has subsequently been renovations NedZink material should be separated
reduced to one fifth of the former values during the last from other materials. Zinc can then easlily be collected
thirty years. for re-use and/or recycling.
As a result of all environmental regulations this amount
will reduce even more in the future, due to the Re-use/Recycling:
reduction of SO 2 concentration in the air. The transfer Scrap produced during the manufacturing process
of zinc ions via rain water is constantly reduced due to
4 Environmental Product Declaration NedZink B.V. – NedZink Naturel
from NedZink material are 100% remelted and fed credits are based on a recycling percentage of 95%
back completely into NedZink's production process. A (European recycling rate for rolled zinc).
small amount of residue (skimmings, dross, dust),
which is no longer valuable for the internal production 2.15 Disposal
process, is completely recycled by a third party Due to the effective recycling process, a maximum of
(European Waste Code 10.05.01). 5% zinc has to be disposed.
The European Wate Code for collected zinc after
The scrap from demolition and renovation work on disassembly is 17.04.04.
building sites is collected and sold either directly to
secondary smelting works or via a scrap metal dealer. 2.16 Further information
The recycling rate for zinc sheets is over 95%. Credits Additional information, optional details, references,
for this recycling are appointed in module D. These data sheets can be obtained at: www.nedzink.com
3. LCA: Calculation rules
3.1 Declared Unit 3.5 Background data
The declared unit is 1 kg of NedZink NATUREL, Background processes are taken from the Ecoinvent
bright-rolled titanium zinc. V3.6 database (2019), with the “allocation, cut-off by
classification” system model.
Declared unit Life cycle inventory data for the production of zinc
Name Value Unit concentrate and SHG Zinc in the Ecoinvent V3.6
Declared unit 1 kg database is updated with the most recent LCA report
conversion factor [Mass/Declared (Zinc Environmental Profile - 2015 Update) on primary
1 -
Unit] Zinc by the International Zinc Association.
Gross density 7200 kg/m3 The environmental impact of the SHG Zinc was then
calculated using SimaPro V9.0. Site-specific data was
provided by NedZink and verified against earlier
studies.
3.2 System boundary
Type of the EPD: Cradle-to-Gate with options. Modules 3.6 Data quality
A1, A2 and A3 contain information on the raw- and The data used for this study was both of high quality
secondary material extraction, transport to the and recent. The specific data was collected by the
manufacturer, manufacturing and packaging. manufacturer, The generic data that is used is less
Only the transport to module C4 is considered under than 10 years old or has been updated within this
module C2. Module C4 takes into account the non- period. This is in compliance with the data quality
recovered zinc at the end of life. Modules A4, A5, B1- requirements of EN 15804.
B7, C1 and C3 are not declared.
Credits after End-of-Life of the product are also 3.7 Period under review
included (module D). Site-specific data for the year 2019 and 2020 was used
in this study. Background data is taken from the
3.3 Estimates and assumptions Ecoinvent V3.6 database (2019) and varies in age.
No major assumptions and estimations were
necessary for the LCA. 3.8 Allocation
Allocation was avoided in this study, as required in EN
3.4 Cut-off criteria 15804. However, in the background database,
No major cut-offs were applied to specific allocation can be applied.
manufacturing data from Nedzink. Production impacts
of packaging for raw materials are not known and 3.9 Comparability
excluded, waste processing of this packaging is known Basically, a comparison or an evaluation of EPD data
and included. For upstream data a background is only possible if all the data sets to be compared
database (Ecoinvent V3.6) was used, which can were created according to EN 15804 and the building
contain additional cut-offs. context, respectively the product-specific
characteristics of performance, are taken into account.
4. LCA: Scenarios and additional technical information
Modules A4, A5, B1-B7, C1 and C3 are not considered
in this study. The possible credits given in Module D
are based on 100% recyclability of zinc products. After End of life (C4) / Recycling potentials (D)
the collection (a collection rate of 95% is taken), zinc Name Value Unit
scrap is re-melted and converted to secondary zinc. Recycling 95% kg
This is not done by NedZink but by third parties. The Landfilling 5% kg
possible credit for the zinc gained through re-melting is
calculated using the dataset of the primary zinc
production. The remaining zinc (5%) is landfilled
(module C4).
5 Environmental Product Declaration NedZink B.V. – NedZink Naturel
5. LCA: Results
DESCRIPTION OF THE SYSTEM BOUNDARY (X = INCLUDED IN LCA; MND = MODULE NOT DECLARED;
MNR = MODULE NOT RELEVANT)
BENEFITS AND
CONSTRUCTI LOADS
PRODUCT STAGE ON PROCESS USE STAGE END OF LIFE STAGE BEYOND THE
STAGE SYSTEM
BOUNDARIES
6 Environmental Product Declaration NedZink B.V. – NedZink Naturel
lairetam
waR
ylppus tropsnarT
gnirutcafunaM
eht
morf
tropsnarT
etis
eht
ot
etag
ylbmessA esU
ecnanetniaM
riapeR
tnemecalpeR tnemhsibrufeR
ygrene
lanoitarepO esu
retaw
lanoitarepO esu
noitcurtsnoc-eD
noitilomed tropsnarT
gnissecorp
etsaW
lasopsiD -esueR -yrevoceR -gnilcyceR laitnetop
A1 A2 A3 A4 A5 B1 B2 B3 B4 B5 B6 B7 C1 C2 C3 C4 D
X X X MND MND MND MND MNR MNR MNR MND MND MND X MND X X
RESULTS OF THE LCA - ENVIRONMENTAL IMPACT according to EN 15804+A1: 1 kg of NEDZINK natural
Parameter Unit A1-A3 C2 C4 D
Global warming potential [kg CO2-Eq.] 3.09E+0 6.52E-4 2.58E-4 -2.37E+0
Depletion potential of the stratospheric ozone layer [kg CFC11-Eq.] 2.38E-7 1.21E-10 8.61E-11 -1.77E-7
Acidification potential of land and water [kg SO2-Eq.] 2.30E-2 2.81E-6 1.89E-6 -1.91E-2
Eutrophication potential [kg (PO4)3--Eq.] 3.24E-3 5.18E-7 3.33E-7 -2.72E-3
Formation potential of tropospheric ozone photochemical
[kg ethene-Eq.] 7.82E-4 9.39E-8 7.92E-8 -6.21E-4
oxidants
Abiotic depletion potential for non-fossil resources [kg Sb-Eq.] 6.78E-2 1.70E-8 2.41E-9 -6.30E-2
Abiotic depletion potential for fossil resources [MJ] 3.54E+1 9.89E-3 7.28E-3 -2.66E+1
RESULTS OF THE LCA - INDICATORS TO DESCRIBE RESOURCE USE according to EN 15804+A1: 1 kg of
NEDZINK natural
Parameter Unit A1-A3 C2 C4 D
Renewable primary energy as energy carrier [MJ] 6.10E+0 1.45E-4 5.95E-5 -4.83E+0
Renewable primary energy resources as material utilization [MJ] 2.64E-1 0.00E+0 0.00E+0 0.00E+0
Total use of renewable primary energy resources [MJ] 6.37E+0 1.45E-4 5.95E-5 -4.83E+0
Non-renewable primary energy as energy carrier [MJ] 4.84E+1 1.07E-2 7.82E-3 -3.78E+1
Non-renewable primary energy as material utilization [MJ] 0.00E+0 0.00E+0 0.00E+0 0.00E+0
Total use of non-renewable primary energy resources [MJ] 4.84E+1 1.07E-2 7.82E-3 -3.78E+1
Use of secondary material [kg] 1.33E-1 0.00E+0 0.00E+0 8.15E-1
Use of renewable secondary fuels [MJ] 0.00E+0 0.00E+0 0.00E+0 0.00E+0
Use of non-renewable secondary fuels [MJ] 0.00E+0 0.00E+0 0.00E+0 0.00E+0
Use of net fresh water [m³] 8.64E-2 1.14E-6 7.86E-6 -7.70E-2
RESULTS OF THE LCA – WASTE CATEGORIES AND OUTPUT FLOWS according to EN 15804+A1:
1 kg of NEDZINK natural
Parameter Unit A1-A3 C2 C4 D
Hazardous waste disposed [kg] 8.63E-3 2.58E-8 1.10E-8 -8.14E-3
Non-hazardous waste disposed [kg] 4.40E-1 6.26E-4 5.00E-2 -3.51E-1
Radioactive waste disposed [kg] 2.19E-4 6.87E-8 4.83E-8 -1.84E-4
Components for re-use [kg] 0.00E+0 0.00E+0 0.00E+0 0.00E+0
Materials for recycling [kg] 0.00E+0 0.00E+0 0.00E+0 0.00E+0
Materials for energy recovery [kg] 0.00E+0 0.00E+0 0.00E+0 0.00E+0
Exported electrical energy [MJ] 0.00E+0 0.00E+0 0.00E+0 0.00E+0
Exported thermal energy [MJ] 0.00E+0 0.00E+0 0.00E+0 0.00E+0
6. LCA: Interpretation
The 7 main impact categories for 1 kg of Nedzink The remaining contributions mainly consist of energy
NATUREL usage (electricity and gas) with a small contribution
from the remaining metal components (Cu, Ti, Al).
Life cycle inventory data for the production of zinc
concentrate and Special High Grade Zinc (SHG Zinc) Because of the high contribution of SHG Zinc and the
in the background database Ecoinvent V3.6 is aligned high recyclability that is assumed, the amount of
with data from the IZA 2015 LCA report (Zinc credits gained in module D for each impact category
Environmetal Profile - 2015 Update, see also section very high, at least 75% or higher compared to the initial
3.5 Background Data). impact value.
The contribution of SHG Zinc is the dominating factor
in all of the impact categories, with contributions >80%
in for all indicators.
7. Requisite evidence
In a literature study TNO-MEP-99/441 of TNO (Dutch The run-off rate is influenced by the atmospheric
Organisation for Applied Scientific Research) the conditions, of which the SO2 concentration is the most
emissions from corrosion of zinc to water have been important variable. With the decreasing of the SO2
evaluated. This corrosion rate refers to the loss of concentration, the corrosion rate is also decreasing.
metallic zinc.
The run-off rate is the wash-off of zinc from the patina In areas with higher SO2-concentration a run-off rate
layer. This run-off rate is generally lower than the off 3 g/m2.yr can be calculated and 2 g/m2.yr in areas
corrosion rate. with lower concentration.
During the built up of the zinc patina layer the run-off is
lower than the corrosion rate. The growth of the patina
layer delays the corrosion.
8. References
General Programme Instructions PCR 2017 Part B
Institut Bauen und Umwelt e.V., Berlin (pub.): The Institut Bauen und Umwelt e.V., Berlin: Product
preparation of environmental product declarations Category Rules for Construction Products from the
(EPDs); General Programme Instructions for the range of Environmental Product Declarations of Institut
preparation of EPDs at the Institut Bauen und Umwelt Bauen und Umwelt (IBU), Part B: Requirements on the
e.V. (IBU), 2016/03 EPD for Building Metals. Version 1.6, November 2017
www.ibu-epd.com www.ibu-epd.com
PCR 2017 Part A EN 988
Institut Bauen und Umwelt e.V., Berlin: Product EN 988:1996
Category Rules for Construction Products from the Zinc and zinc alloys - Specification for rolled flat
range of Environmental Product Declarations of Institut products for building
Bauen und Umwelt (IBU), Part A: Calculation Rules for
the Life Cycle Assessment and Requirements on the EN 1179
Background Report. Version 1.8, July 2019 EN 1179:2003
www.ibu-epd.com Zinc and zinc alloys - Primary zinc
7 Environmental Product Declaration NedZink B.V. – NedZink Naturel
EN 612
EN 612:2005 ISO 15686
Eaves gutters with bead stiffened fronts and rainwater ISO 15686
pipes with seamed joints made of metal sheet Buildings and constructed assets - Service life
planning
EN 13501-1
EN 13501-1:2007+A1:2009 96/603/EC
Fire classification of construction products and building EU Commission Decision of 4 October 1996
elements - Part 1: Classification using data from establishing the list of products belonging to Classes A
reaction to fire tests 'No contribution to fire' provided for in Decision
94/611/EC implementing Article 20 of Council Directive
EN 13501-5 89/106/EEC on construction products (Text with EEA
EN 13501-5:2006+A1:2009 relevance)
Fire classification of construction products and building
elements - Part 5: Classification using data from KOMO product certificates
external fire exposure to roofs tests BRL2034: K7054/04 zinc sheets
BRL2035: K7057/04 zinc gutters
EN 14782 BRL2044: K7063/04 zinc downpipes
EN 14782:2006
Self-supporting metal sheet for roofing, external Lloyd's Register Product certificate (approval No
cladding and internal lining - Product specification and QIS 122)
requirements Lloyd’s Register Inspection Services - Product
certificate Industrial Quality Scheme for Product
EN 14783 Certification by Surveillance of Quality Systems
EN 14783:2013 (approval No QIS 122)
Fully supported metal sheet and strip for roofing,
external cladding and internal lining - Product Candidate List of substances of very high concern
specification and requirements for Authorisation
ECHA published in accordance with Article 59(10) of
EN 15804 the REACH Regulation (2018)
EN 15804:2012-04+A1:2013
Sustainability of construction works - Environmental TNO-MEP-99/441
Product Declarations - Core rules for the product Diffusive Emissions of zinc due to atmospheric
category of construction products corrosion of zinc and zinc coated (galvanised)
materials - R.H.J. Korenromp, J.C.Th. Hollander
DIN 4102 (1999)
DIN 4102
Fire behaviour of building materials and building Zinc Environmental Profile - 2015 Update
components International Zinc Association (2016)
ISO 9001 Zinc Recycling, Closing the Loop
ISO 9001:2015 International Zinc Association (2011)
Quality management systems - Requirements
Zinc…A Sustainable Material
ISO 14001 International Zinc Association (2010)
ISO 14001:2015
Environmental management systems - Requirements Zinc, A Sustainable Material – Essential for Modern
with guidance for use Life.
International Zinc Association (2017)
ISO 14025
ISO 14025:2011-10 SimaPro V9.0
Environmental labels and declarations - Type III Life Cycle Assessment software
environmental declarations - Principles and procedures
Ecoinvent V3.6
ISO 14040 Life Cycle Inventory database, 2019
ISO 14040:2006
Environmental management - Life cycle assessment -
Principles and framework
ISO 14044
ISO 14044:2006
Environmental management - Life cycle assessment -
Requirements and guidelines
8 Environmental Product Declaration NedZink B.V. – NedZink Naturel
Publisher
Institut Bauen und Umwelt e.V. Tel +49 (0)30 3087748- 0
Panoramastr. 1 Fax +49 (0)30 3087748- 29
10178 Berlin Mail info@ibu-epd.com
Germany Web www.ibu-epd.com
Programme holder
Institut Bauen und Umwelt e.V. Tel +49 (0)30 - 3087748- 0
Panoramastr 1 Fax +49 (0)30 – 3087748 - 29
10178 Berlin Mail info@ibu-epd.com
Germany Web www.ibu-epd.com
Author of the Life Cycle
Assessment Tel +31 (0)30-693 00 55
Stichting Adviescentrum Metaal Fax +31 (0)30-693 00 57
Kelvinbaan 40 Mail info@metaaladvies.nl
3430MT Nieuwegein Web metaaladvies.nl
Netherlands
Owner of the Declaration
NedZink B.V. Tel +31 (0)475 455700
Hoofdstraat 1 Fax +31 (0)475 455790
6024AA Budel-Dorplein Mail info@nedzink.com
Netherlands Web www.nedzink.com
