ENVIRONMENTAL PRODUCT DECLARATION
as per ISO 14025 and EN 15804+A2
Owner of the Declaration dormakaba International Holding GmbH
Publisher Institut Bauen und Umwelt e.V. (IBU)
Programme holder Institut Bauen und Umwelt e.V. (IBU)
Declaration number EPD-DOR-20230248-CBA1-EN
Issue date 01.07.2023
Valid to 30.06.2028
Saffire LX Series
dormakaba
www.ibu-epd.com | https://epd-online.com
General Information
dormakaba Saffire LX Series
Programme holder Owner of the declaration
IBU – Institut Bauen und Umwelt e.V. dormakaba International Holding GmbH
Hegelplatz 1 DORMA Platz 1
10117 Berlin 58256 Ennepetal
Germany Germany
Declaration number Declared product / declared unit
EPD-DOR-20230248-CBA1-EN 1 piece of the product: Mortise Lock Saffire LX-M, consisting of the
following items:
• Mortise Lock Saffire LX-M
• Lever handle
• Fixing materials
• Product packaging
This declaration is based on the product category rules: Scope:
Electronic and physical Access Control Systems, 01.08.2021 This Environmental Product Declaration refers to a specific mortise lock
(PCR checked and approved by the SVR) manufactured by dormakaba. The EPD is representative for the Saffire LX
Series. The production site is located in Montreal (Canada).
Issue date Data represents the year 2022.
01.07.2023
The owner of the declaration shall be liable for the underlying information
and evidence; the IBU shall not be liable with respect to manufacturer
information, life cycle assessment data and evidences.
Valid to
30.06.2028 The EPD was created according to the specifications of EN 15804+A2. In
the following, the standard will be simplified as EN 15804.
Verification
The standard EN 15804 serves as the core PCR
Independent verification of the declaration and data according to ISO
14025:2011
internally X externally
Dipl.-Ing. Hans Peters
(Chairman of Institut Bauen und Umwelt e.V.)
Florian Pronold Matthias Klingler,
(Managing Director Institut Bauen und Umwelt e.V.) (Independent verifier)
1 Environmental Product Declaration - dormakaba - Saffire LX Series
Product
The products are not harmonised in accordance with the
Product description/Product definition Construction Product Regulations (CPR) but in accordance with
The Saffire LX-M Mortise Lock is a sleek, contemporary Radio other provisions for harmonisation of the EU. Compliance with
Frequency Identification (RFID) lock with a small footprint the European Union Directive and technical specifications:
designed with the latest connectivity and security conveniences
for multi-housing properties. The Saffire LX-M provides an • Directive (EU) No 2011/65 (RoHS)
easy-to-use, secure, and flexible solution. With its sleek curves • Regulation (EC) No 1907/2006 (REACH)
and clean aesthetics, Saffire LX-M results in a lock design that • ANSI A156.13
integrates seamlessly with your property décor. • ANSI A156.25
• UL 10C
The mortise lock is equipped with Bluetooth Low Energy (BLE) • ULC S-104
Technology, which gives today's residents the added • EN 12209
convenience of using a smart device in addition to RFID fobs • EN 1634-1
for access units, common areas and the perimeter. Our key • EN 1363-1
delivery platform issues and authenticates mobile credentials
through BlueSky, dormakaba's mobile access app.
Base materials/Ancillary materials
For the use and application of the product the representative The major material composition including the packaging of the
national provisions apply. For the Saffire LX Series, the product is listed below:
standards which can be applied are the following: Name Value Unit
• ANSI A156.13 Steel 43 %
• ANSI A156.25 Zinc 38 %
• UL 10C
Paper 13 %
• ULC S-104
Electronics 3 %
• EN 12209
• EN 1634-1 Plastics 2 %
• EN 1363-1 The product includes partial articles which contain substances
listed in the Candidate List of REACH Regulation
1907/2006/EC (date: 17.01.2023) exceeding 0.1 percentage by
Application
mass: no
The Saffire LX series is the ideal application for:
• New construction projects The Candidate List can be found on the ECHA website:
• Areas where doors are being replaced https:echa.europa.eu/de/home.
• Access control for resident units and common areas
• Mulithousing properties Reference service life
• Hotels The reference service life for the Saffire LX Series amounts to
10 years, depending on the application and frequency of use.
For repairs and renewals, suitable spare parts are available.
Technical Data The mortise lock series is tested and certified to BHMA
A156.13, meaning they are designed to withstand a minimum
of 1.000.000 cycles.
The Saffire LX-M Mortise Lock series has the following
technical properties:
Name Value Unit
Electronic mortise lock set with contactless
1 piece
RFID reader
Handling left/rightreversible
Door Thickness max. 66 mm
Standard Backset 70 mm
Batteries 3 AA
Mobile Access BLE enabled
Audit memory 4000 events
LCA: Calculation rules
Declared Unit System boundary
The declared unit is 1 piece of the product: Saffire LX-M The type of EPD is: cradle to gate with options, modules C1–
Name Value Unit C4, and module D (A1–A3 + C + D and additional modules: A4
+ A5 + B2)
Declared unit 1 pce.
Mass reference of declared product 3,75 kg/pce
2 Environmental Product Declaration - dormakaba - Saffire LX Series
Production - Modules A1-A3 Module D (Benefits and loads beyond the system boundary)
The product stage includes: includes:
— A1, raw material extraction, processing and mechanical — D, recycling potentials, expressed as net impacts and
treatments, processing of secondary material input (e.g. benefits.
recycling processes), — A2, transport to the manufacturer,
— A3, manufacturing and assembly including provision of all Geographic Representativeness
materials, products and energy, as well as waste processing up Land or region, in which the declared product system is
to the end-of-waste state. manufactured, used or handled at the end of the product´s
lifespan: Global
Construction stage - Modules A4-A5
The construction process stage includes:
Comparability
— A4, transport to the building site;
Basically, a comparison or an evaluation of EPD data is only
— A5, installation into the building;
possible if all the data sets to be compared were created
including provision of all materials, products and energy, as well
according to EN 15804 and the building context, respectively
as waste processing up to the end-of-waste state or disposal of
the product-specific characteristics of performance, are taken
final residues during the construction process stage.
into account. GaBi, SP40
Maintenance – Module B2
This module includes the production and the end of life of the
batteries. The potential use of batteries is declared in module
B2.
End-of-life stage– Modules C1-C4 and D
The end-of-life stage includes:
— C1, de-construction, demolition:
— C2, transport to waste processing;
— C3, waste processing for reuse, recovery and/or recycling;
— C4, disposal;
including provision and all transport, provision of all materials,
products and related energy and water use.
LCA: Scenarios and additional technical information
are provided by dormakaba. During the operation of the
Characteristic product properties of biogenic carbon product, the only energy consumption comes from the battery
Information on describing the biogenic Carbon Content at use. The battery must be exchanged on average 5 times over
factory gate the declared service life. In order to allow scaling, the exchange
of 1 battery is declared in the LCA.
Name ValueUnit
Biogenic carbon content in accompanying kg
0,17 Reference service life
packaging C
Name Value Unit
Note: 1 kg of biogenic carbon is equivalent to 44/12 kg of CO .
2 Life Span according to the manufacturer 10 a
End of life (C1-C4)
C1: The product dismantling from the building is done manually
Transport to the building site (A4) without environmental burden.
Name Value Unit C2: Transport to waste management: 50 km.
Litres of fuel 0.00276l/100km Name Value Unit
Capacity utilisation (including empty runs) via Collected separately waste type 3.28 kg
55 %
medium truck Recycling 3.12 kg
Transport distance via medium truck 100 km Energy recovery 0.0635 kg
The product is transported via truck. The product is stored in Landfilling 0.092 kg
the dormakaba logistic centre in Montreal. The main distribution The product is disassembled in a recycling process. Material
region is North America. In order to allow scaling to a specific recycling is then assumed for the metals and electronics. The
point of installation 100 km are declared. plastic components are assumed to be incinerated with energy
recovery. Minor proportions of residues arising from the
Installation into the building (A5) recycling process are landfilled. Region for the End of Life is:
Global.
Name Value Unit
Waste packaging (paper) 0,471 kg
Reuse, recovery and/or recycling potentials (D), relevant
Maintenance (B2) scenario information
Name Value Unit Name Value Unit
Use of batteries 5 pieces Recycling 100 %
dormakaba Mortise Lock Saffire LX series are operated using a The collection rate is 100 %.
battery and are not connected to mains electricity. The batteries
3 Environmental Product Declaration - dormakaba - Saffire LX Series
LCA: Results
DESCRIPTION OF THE SYSTEM BOUNDARY (X = INCLUDED IN LCA; MND = MODULE OR INDICATOR NOT DECLARED; MNR
= MODULE NOT RELEVANT)
Benefits and
Construction loads beyond
Product stage Use stage End of life stage
process stage the system
boundaries
la ire ta m w a Ry lp p u s tro p s n a rT g n iru tc a fu n a M e h t m o rf tro p s n a rTe tis e h t o t e ta g y lb m e s s A e s U e c n a n e tn ia M ria p e R tn e m e c a lp e R tn e m h s ib ru fe R y g re n e la n o ita re p Oe s u re ta w la n o ita re p Oe s u n o itc u rts n o c -e Dn o itilo m e d tro p s n a rT g n is s e c o rp e ts a W la s o p s iD -e s u e R-y re v o c e R-g n ilc y c e Rla itn e to p
A1 A2 A3 A4 A5 B1 B2 B3 B4 B5 B6 B7 C1 C2 C3 C4 D
X X X X X MND X MNR MNR MNR MND MND X X X X X
RESULTS OF THE LCA - ENVIRONMENTAL IMPACT according to EN 15804+A2: 1 piece Saffire LX Series
Parameter Unit A1-A3 A4 A5 B2 C1 C2 C3 C4 D
GWP-total kg CO 2 eq 1.04E+01 3.3E-02 6.68E-01 2.09E-01 0 1.4E-02 2.38E-01 1E-03 -6.15E+00
GWP-fossil kg CO 2 eq 1.11E+01 3.1E-02 1.7E-02 2.09E-01 0 1.4E-02 2.38E-01 1E-03 -6.14E+00
GWP-biogenic kg CO 2 eq -7.2E-01 1E-03 6.51E-01 2.88E-04 0 6.31E-04 5.54E-06 4.77E-06 -7E-03
GWP-luluc kg CO 2 eq 1.4E-02 7.46E-07 1.1E-05 8.67E-05 0 3.25E-07 1.34E-05 4.02E-06 -6E-03
ODP kg CFC11 eq 1.39E-10 3.31E-18 1.2E-16 7.19E-16 0 1.44E-18 1.2E-16 5.18E-18 -2.82E-14
AP mol H+ eq 5.3E-02 3.14E-05 1.87E-04 2.11E-03 0 1.37E-05 4.23E-05 1E-05 -2.9E-02
EP-freshwater kg P eq 4.89E-05 6.7E-09 2.35E-08 1.48E-07 0 2.92E-09 1.91E-08 2.4E-09 -1.5E-05
EP-marine kg N eq 8.89E-03 9.98E-06 6.75E-05 2.54E-04 0 4.35E-06 9.54E-06 2.58E-06 -4E-03
EP-terrestrial mol N eq 1.04E-01 1.11E-04 8.42E-04 2.32E-03 0 4.84E-05 1.93E-04 2.83E-05 -4.3E-02
kg NMVOC
POCP 2.8E-02 2.82E-05 1.79E-04 7.85E-04 0 1.23E-05 2.64E-05 7.8E-06 -1.4E-02
eq
ADPE kg Sb eq 6.05E-03 9.39E-10 1.9E-09 9.05E-06 0 4.1E-10 1.64E-09 1.25E-10 -2E-03
ADPF MJ 1.6E+02 4.44E-01 2.11E-01 2.37E+00 0 1.94E-01 1.1E-01 1.8E-02 -7.87E+01
m3 world eq
WDP 3.77E+00 6.14E-05 8.3E-02 2.3E-02 0 2.68E-05 2.4E-02 1.46E-04 -1.52E+00
deprived
GWP = Global warming potential; ODP = Depletion potential of the stratospheric ozone layer; AP = Acidification potential of land and water; EP =
Eutrophication potential; POCP = Formation potential of tropospheric ozone photochemical oxidants; ADPE = Abiotic depletion potential for non-fossil
resources; ADPF = Abiotic depletion potential for fossil resources; WDP = Water (user) deprivation potential)
RESULTS OF THE LCA - INDICATORS TO DESCRIBE RESOURCE USE according to EN 15804+A2: 1 piece Saffire LX Series
Parameter Unit A1-A3 A4 A5 B2 C1 C2 C3 C4 D
PERE MJ 6.06E+01 1E-03 5.69E+00 1.97E-01 0 6.11E-04 2.9E-02 2E-03 -1.68E+01
PERM MJ 5.65E+00 0 -5.65E+00 0 0 0 0 0 0
PERT MJ 6.62E+01 1E-03 3.8E-02 1.97E-01 0 6.11E-04 2.9E-02 2E-03 -1.68E+01
PENRE MJ 1.58E+02 4.45E-01 2.11E-01 2.37E+00 0 1.94E-01 2.21E+00 1.8E-02 -7.87E+01
PENRM MJ 2.1E+00 0 0 0 0 0 -2.1E+00 0 0
PENRT MJ 1.6E+02 4.45E-01 2.11E-01 2.37E+00 0 1.94E-01 1.1E-01 1.8E-02 -7.87E+01
SM kg 1.59E+00 0 0 0 0 0 0 0 0
RSF MJ 0 0 0 0 0 0 0 0 0
NRSF MJ 0 0 0 0 0 0 0 0 0
FW m3 1.11E-01 2.51E-06 2E-03 7.23E-04 0 1.1E-06 5.81E-04 4.62E-06 -5.3E-02
PERE = Use of renewable primary energy excluding renewable primary energy resources used as raw materials; PERM = Use of renewable primary
energy resources used as raw materials; PERT = Total use of renewable primary energy resources; PENRE = Use of non-renewable primary energy
excluding non-renewable primary energy resources used as raw materials; PENRM = Use of non-renewable primary energy resources used as raw
materials; PENRT = Total use of non-renewable primary energy resources; SM = Use of secondary material; RSF = Use of renewable secondary fuels;
NRSF = Use of non-renewable secondary fuels; FW = Use of net fresh water
RESULTS OF THE LCA – WASTE CATEGORIES AND OUTPUT FLOWS according to EN 15804+A2:
1 piece Saffire LX Series
Parameter Unit A1-A3 A4 A5 B2 C1 C2 C3 C4 D
HWD kg 2.1E-06 4.31E-11 3.11E-10 1.15E-08 0 1.88E-11 4.2E-10 2.79E-10 -1.85E-06
NHWD kg 8.2E-01 4.55E-05 2.1E-02 1E+00 0 1.98E-05 2.5E-02 9.2E-02 1.7E-02
RWD kg 1.1E-02 4.77E-07 1.11E-05 4.87E-05 0 2.08E-07 4.09E-06 2.09E-07 -3E-03
CRU kg 0 0 0 0 0 0 0 0 0
MFR kg 0 0 0 0 0 0 3.08E+00 0 0
MER kg 0 0 0 0 0 0 0 0 0
EEE MJ 0 0 1.01E+00 0 0 0 4.51E-01 0 0
EET MJ 0 0 1.83E+00 0 0 0 1.04E+00 0 0
4 Environmental Product Declaration - dormakaba - Saffire LX Series
HWD = Hazardous waste disposed; NHWD = Non-hazardous waste disposed; RWD = Radioactive waste disposed; CRU = Components for re-use;
MFR = Materials for recycling; MER = Materials for energy recovery; EEE = Exported electrical energy; EET = Exported thermal energy
RESULTS OF THE LCA – additional impact categories according to EN 15804+A2-optional:
1 piece Saffire LX Series
Parameter Unit A1-A3 A4 A5 B2 C1 C2 C3 C4 D
Disease
PM 6.25E-07 1.65E-10 1.04E-09 7.58E-08 0 7.19E-11 5.4E-10 1.24E-10 -4.07E-07
incidence
IR kBq U235 eq 1.17E+00 6.82E-05 2E-03 5.24E-03 0 2.97E-05 3.68E-04 2.15E-05 -4.07E-01
ETP-fw CTUe 8.38E+01 3.15E-01 1E-01 6.06E-01 0 1.37E-01 4.1E-02 1E-02 -3.6E+01
HTP-c CTUh 4.58E-07 5.92E-12 5.29E-12 9.7E-11 0 2.58E-12 3.58E-12 1.55E-12 1.6E-08
HTP-nc CTUh 7.55E-07 2.53E-10 2.29E-10 3.41E-09 0 1.1E-10 3.62E-10 1.71E-10 2.16E-06
SQP SQP 1.28E+02 1E-03 5.6E-02 4.61E-01 0 4.98E-04 3.3E-02 4E-03 -6.39E+00
PM = Potential incidence of disease due to PM emissions; IR = Potential Human exposure efficiency relative to U235; ETP-fw = Potential comparative
Toxic Unit for ecosystems; HTP-c = Potential comparative Toxic Unit for humans (cancerogenic); HTP-nc = Potential comparative Toxic Unit for humans
(not cancerogenic); SQP = Potential soil quality index
Disclaimer 1 – for the indicator IRP
This impact category deals mainly with the eventual impact of low-dose ionizing radiation on human health of the nuclear fuel cycle. It
does not consider effects due to possible nuclear accidents, occupational exposure or radioactive waste disposal in underground
facilities. Potential ionizing radiation from the soil, from radon and from some construction materials is also not measured by this
indicator.
Disclaimer 2 – for the indicators ADPE, ADPF, WDP, ETP-fw, HTP-c, HTP-nc, SQP
The results of this environmental impact indicator shall be used with care as the uncertainties on these results are high as there is
limited experience with the indicator. This EPD was created using a software tool.
References
ANSI A156.25:2023
ANSI A156.25:2023, Electrified Locking Devices ROHS3 Directive
Directive on the restriction of the use of certain hazardous
ANSI A156.13:2022 substances in electrical and electronic equipment (RoHS),
ANSI A156.13:2022, Mortise Locks Directive (EU) No 2011/65
UL 10C:2016 Further References
UL 10C:2016-06, Standard for Safety Positive Pressure Fire
Tests of Door Assemblies IBU 2021
General Instructions for the EPD programme of Institut Bauen
ULC CAN-S104:2020 und Umwelt e.V. Version 2.0, Berlin: Institut Bauen und Umwelt
ULC CAN-S104:2020-08, Standard Method for Fire Tests of e.V., 2021. www.ibu-epd.com
Door Assemblies
GaBi
EN 12209:2016 Sphera Solutions GmbH
EN 12209:2016, Building hardware - Mechanically operated Gabi Software System and Database for Life Cycle
locks and locking plates - Requirements and test methods Engineering 1992-2020
Version 10.0.0.71
EN 1634-1:2018 University of Stuttgart
EN 1634-1:2018-04, Fire resistance and smoke control tests for Leinfelden-Echterdingen
door and shutter assemblies, openable windows and elements
of building hardware GaBi ts documentation
GaBi life cycle inventory data documentation
DIN EN 1363-1:2020-05 (https://www.gabi-software.com/support/gabi/gabidatabase-
DIN EN 1363-1:2020-05, Fire resistance tests - Part 1: General 2020-lci-documentation/).
requirements
LCA-tool dormakaba
DIN EN ISO 14025: LCA tool, ESC
DIN EN ISO 14025:2011-10, LCA-Tool No.: IBU-DOR-202109-LT1-EN.
Environmental labels and declarations — Type III Developed by Sphera Solutions GmbH
environmental declarations - Principles and procedures
PCR Part A
EN 15804:2019+A2 PCR – Part A: Calculation Rules for the Life Cycle Assessment
EN 15804:2019+A2 (in press), Sustainability of construction and Requirements on the Project Re-port
works — Environmental Product Declarations — Core rules for according to EN 15804+A2:2019, Version 1.0, Institut
the product category of Bauen und Umwelt e.V., www.ibu-epd.com.
construction products.
PCR Part B
REACH PCR – Part B: Requirements on the EPD for Building
Regulation (EC) No 1907/2006 of the European Parliament and Hardware product, version 1.2, Institut Bauen und
of the Council on the Registration, Evaluation, Authorisation Umwelt e.V., www.ibu-epd.com, 2019.
and Restriction of Chemicals
5 Environmental Product Declaration - dormakaba - Saffire LX Series
Publisher
Institut Bauen und Umwelt e.V. +49 (0)30 3087748- 0
Hegelplatz 1 info@ibu-epd.com
10117 Berlin www.ibu-epd.com
Germany
Programme holder
Institut Bauen und Umwelt e.V. +49 (0)30 3087748- 0
Hegelplatz 1 info@ibu-epd.com
10117 Berlin www.ibu-epd.com
Germany
Author of the Life Cycle Assessment
dormakaba International Holding GmbH +49 2333 793-0
DORMA Platz 1 info.de@dormakaba.com
58256 Ennepetal www.dormakaba.com
Germany
Owner of the Declaration
dormakaba International Holding GmbH +49 2333 793-0
DORMA Platz 1 info.de@dormakaba.com
58256 Ennepetal www.dormakaba.com
Germany
6 Environmental Product Declaration - dormakaba - Saffire LX Series
