ENVIRONMENTAL PRODUCT DECLARATION
as per ISO 14025 and EN 15804+A2
Owner of the Declaration Kingspan Insulation B.V.
Programme holder Institut Bauen und Umwelt e.V. (IBU)
Publisher Institut Bauen und Umwelt e.V. (IBU)
Declaration number EPD-KSI-20210042-CBA1-EN
Issue date 24.03.2021
Valid to 23.03.2026
Kooltherm® K17
Kingspan Insulation B.V.
www.ibu-epd.com | https://epd-online.com
Umwelt Produktdeklaration Name des Herstellers – Name des Produkts
General Information
Kingspan Insulation B.V. Kooltherm® K17
Programme holder Owner of the declaration
IBU – Institut Bauen und Umwelt e.V. Kingspan Insulation B.V.
Panoramastr. 1 Lingewei 8
10178 Berlin 4004 LL Tiel
Germany The Netherlands
Declaration number Declared product / declared unit
EPD-KSI-20210042-CBA1-EN Kooltherm® K17 Inner Wall Board
1 m2, 100/12,5 mm thickness, R = 5,05 m²·K/W
D
This declaration is based on the product Scope:
category rules: The insulation material Kooltherm® is produced by
Insulating materials made of foam plastics, 06.2017 Kingspan Insulation B.V. at the manufacturing facility in
(PCR checked and approved by the SVR) Tiel, the Netherlands. A glass tissue based facing
(backside) and a composite foil based facing (frontsite)
is autohesively bonded to the insulation core during
Issue date
manufacture. On the frontside a gypsum plasterboard
24.03.2021
is bonded afterwards.
Valid to
In order to enable the user of the EPD to calculate the
23.03.2026
LCA results for different thicknesses, the EPD contains
the respective calculation rules.
The owner of the declaration shall be liable for the
underlying information and evidence; the IBU shall not
be liable with respect to manufacturer information, life
cycle assessment data and evidences.
The EPD was created according to the specifications
of EN 15804+A2. In the following, the standard will be
simplified as EN 15804.
Verification
The standard EN 15804 serves as the core PCR
Independent verification of the declaration and data
according to ISO 14025:2010
Dipl. Ing. Hans Peters internally x externally
(chairman of Institut Bauen und Umwelt e.V.)
Dr. Alexander Röder Dipl. Natw. ETH Sascha Iqbal
(Managing Director Institut Bauen und Umwelt e.V.)) (Independent verifier)
Product
Product description/Product definition CE-marking. For the application and use the respective
Kooltherm® K17 is a rigid thermoset cellular insulation national provisions apply.
material faced with a glass tissue facing on the
backside and a composite foil based facing on the Application
frontsite. On the frontside a gypsum plasterboard (12,5 Due to its high insulating value, Kooltherm® K17 is
mm) is bonded. The product is available in variable suitable for use as inner wall insulation and can be
thicknesses from 20/12,5 mm up to 200/12,5 mm. This used for renovation projects.
EPD covers one of the most commonly sold thickness
of 100/12,5 mm with an R -value of 5,05 m²·K/W. Technical Data
D
For the placing on the market of the product in the
European Union/European Free Trade Association Constructional data
(EU/EFTA) (with the exception of Switzerland) Name Value Unit
Regulation (EU) No. 305/2011 (CPR) applies. The Compressive strength acc. to EN
≥ 100 kPa
product needs a declaration of performance taking into 13166
consideration EN 13166:2012+A2:2016 - Thermal Thermal conductivity λd acc. to EN
0.021 W/(mK)
insulation products for buildings - Factory made 13166 for d = 20 – 44 mm
phenolic foam (PF) products - Specification and the Thermal conductivity λd acc. to EN 0.020 W/(mK)
2 Environmental Product Declaration Kingspan Insulation B.V. – Kooltherm® K17
13166 for d = 45 – 120 mm the requirements of Article 57 and 59(1)
Thermal conductivity λd (gypsum of REACH Regulation (EC) No 1907/2006. These
plasterboard) acc. to EN 13950 for d = 0.25 W/(mK) products are not classified as “hazardous products”
12.5 mm according to any current legislation, and can hence be
Technical parameters not included are modulus of declared as follows:
elasticity as well as sound absorption (not relevant for - This article contains substances listed in the
this application), and creep (not placed under candidate list (date: 19.01.2021) exceeding 0.1
permanent load). percentage by mass: no.
- This article contains other carcinogenic, mutagenic,
Performance data of the product in accordance with reprotoxic (CMR) substances in categories 1A or 1B
the declaration of performance with respect to its which are not on the candidate list, exceeding 0.1
essential characteristics according to EN percentage by mass: no.
13166:2012+A2:2016 - Thermal insulation products for - Biocide products were added to this construction
buildings - Factory made phenolic foam (PF) products - product or it has been treated with biocide products
Specification (this then concerns a treated product as defined by the
(EU) Biocidal Products Regulation No. 528/2012
Base materials/Ancillary materials (BPR): no.
The main materials are phenolic (PF) resin (between
70-80%) with added catalyst and additives (between The chemical functional group of the additives used in
15-20%). Phenolic rigid foam onto a facing material the resin is that of non-ionic surfactants.
(between 5-10%) is formed by the chemical reaction of
these materials and adding a blowing agent with no Reference service life
ozone depletion potential (ca. 5%). Due to the closed- The reference service life is not to be declared in this
cell structure (conform EN 13166), the blowing agent EPD as it does not cover the use stage.
remains in the foam. In the
current REACH regulations, phenolic foam insulation
products are considered “articles” and are exempt from
LCA: Calculation rules
Declared Unit · A5 installation in the building
The declared unit (1 m²) and conversion factors are including provision of all materials, products and
listed in the table below. energy, as well as waste processing up to the end-of-
waste state or disposal of final residues during the
Declared unit construction process stage.
Name Value Unit
Declared unit thickness 100/12.5 The end-of-life stage is a mandatory information
1 m2
mm module and it covers:
Gross density 103.1 kg/m3 · C1 de-construction, demolition;
conversion factor [Mass/Declared · C2 transport to waste processing;
12.9 -
Unit] ( in kg/m² ) · C3 waste processing for reuse, recovery and/or
Grammage 12.9 kg/m2 recycling;
Layer thickness 0.125 m · C4 disposal (not applicable for this EPD)
including provision and all transport, provision of all
materials, products and related energy and water use.
System boundary Environmental burden of the incineration (R1 > 60%)
Type of EPD: according to EN 15804: of the product
cradle to gate with options, modules C1–C4, and at the end-of-life stage are assigned to the product
module D (A1–A3, C, D and additional modules: system (C3); resulting potential credits for thermal and
A4,A5). electrical energy from energy substitution are declared
in module D.
According to PCR Part A:
1a) declaration of one specific product from one plant Renewable electricity sources for manufacturing
of one manufacturer; All electricity used during production comes from
renewable sources.
The product stage is a mandatory information module By generating energy on-site with solar panels and
and it covers: with procured energy from fully certified renewable
· A1, raw material extraction and processing, sources. Following the global Net Zero Energy strategy
processing of secondary material input (e.g. recycling from Kingspan Group plc.
processes),
· A2, transport to the manufacturer, Comparability
· A3, manufacturing, Basically, a comparison or an evaluation of EPD data
including provision of all materials, products and is only possible if all the data sets to be compared
energy, packaging processing and its transport, as well were created according to EN 15804 and the building
as waste processing up to the end-of-waste state or context, respectively the product-specific
disposal of final residues during the product stage. characteristics of performance, are taken into account.
The construction process stage includes: Factors for different thicknesses
· A4 transport to the building site;
3 Environmental Product Declaration Kingspan Insulation B.V. – Kooltherm® K17
The LCA results for the insulation material declared in following table can be used for the calculation. For
this EPD refer to a product with a thickness of 100/12,5 modules A1- A3, C3 and D the LCA results in chapter
mm. To enable the user of the EPD to calculate the 5 have to be multiplied with these factors.
results for different thicknesses the factors in the
Background data from GaBi software-system version
9 with Service Packs 39 GaBi ts is used.
LCA: Scenarios and additional technical information
Characteristic product properties Collected as mixed construction waste 11.6 kg
Information on biogenic Carbon Energy recovery 11.6 kg
The total mass of biogenic carbon containing materials R1-value of waste incineration plant >60 %
is less than 5 % of the total mass of the product and
accompanying packaging.
Reuse, recovery and/or recycling potentials (D),
relevant scenario information
Technical information Waste incineration with energy recuperation is
The following technical information is a basis for the assumed as end-of life scenario
declared modules or can be used for developing
specific scenarios in the context of a building
assessment.
Transport to the building site (A4)
Name Value Unit
Litres of fuel 0.0103 l/100km
Transport distance 100 km
Gross density of products transported 103.1 kg/m3
Installation into the building (A5)
Name Value Unit
Output substances following waste
0.08 kg
treatment on site packaging material
Within A1-A3 the following packaging of the final
product is included:
Polyethylene cover and wrap: 0,06 kg/m²
Others (mainly Expanded Polystyrene skid): 0,02
kg/m²
The recycling of the packaging is considered in A5.
End of life (C1-C4)
The assumptions for C1 are: diesel driven excavator
(100 kW; 0.2 litre fuel per ton excavated material).
The assumptions for C2 are: Truck Euro 6, diesel
driven, 26-28 t gross weight, assumed distance 50 km
Name Value Unit
4 Environmental Product Declaration Kingspan Insulation B.V. – Kooltherm® K17
LCA: Results
Disclaimer:
EP-freshwater: This indicator has been calculated as “kg P eq” as required in the characterization model
(EUTREND model, Struijs et al., 2009b, as implemented in ReCiPe;
http://eplca.jrc.ec.europa.eu/LCDN/developerEF.xhtml)
Disclaimer:
EP-freshwater: This indicator has been calculated as “kg P eq” as required in the characterization model
(EUTREND model, Struijs et al., 2009b, as implemented in ReCiPe;
http://eplca.jrc.ec.europa.eu/LCDN/developerEF.xhtml).
DESCRIPTION OF THE SYSTEM BOUNDARY (X = INCLUDED IN LCA; ND = MODULE OR INDICATOR NOT
DECLARED; MNR = MODULE NOT RELEVANT)
BENEFITS AND
CONSTRUCTI LOADS
PRODUCT STAGE ON PROCESS USE STAGE END OF LIFE STAGE BEYOND THE
STAGE SYSTEM
BOUNDARIES
5 Environmental Product Declaration Kingspan Insulation B.V. – Kooltherm® K17
lairetam
waR
ylppus tropsnarT
gnirutcafunaM
eht
morf
tropsnarT
etis
eht
ot
etag
ylbmessA esU
ecnanetniaM
riapeR
tnemecalpeR tnemhsibrufeR
ygrene
lanoitarepO esu
retaw
lanoitarepO esu
noitcurtsnoc-eD
noitilomed tropsnarT
gnissecorp
etsaW
lasopsiD -esueR -yrevoceR -gnilcyceR laitnetop
A1 A2 A3 A4 A5 B1 B2 B3 B4 B5 B6 B7 C1 C2 C3 C4 D
X X X X X ND ND MNR MNR MNR ND ND X X X X X
RESULTS OF THE LCA - ENVIRONMENTAL IMPACT according to EN 15804+A2: 1 m2 100/12,5 mm
thickness
Core Indicator Unit A1-A3 A4 A5 C1 C2 C3 C4 D
GWP-total [kg CO2-Eq.] 1.06E+1 9.85E-2 2.00E-1 7.44E-3 4.93E-2 2.56E+1 0.00E+0 -1.08E+1
GWP-fossil [kg CO2-Eq.] 1.04E+1 9.76E-2 2.00E-1 7.44E-3 4.88E-2 2.56E+1 0.00E+0 -1.08E+1
GWP-biogenic [kg CO2-Eq.] 4.55E-2 -5.94E-4 -3.63E-6 -5.24E-7 -2.97E-4 1.15E-3 0.00E+0 -2.09E-2
GWP-luluc [kg CO2-Eq.] 7.63E-2 1.49E-3 7.20E-6 2.52E-7 7.47E-4 2.48E-4 0.00E+0 -7.34E-3
ODP [kg CFC11-Eq.] 1.25E-8 1.19E-17 5.97E-17 7.14E-19 5.93E-18 3.07E-15 0.00E+0 -1.10E-13
AP [mol H+-Eq.] 4.69E-2 1.15E-4 2.76E-5 3.54E-5 5.76E-5 1.53E-2 0.00E+0 -2.03E-2
EP-freshwater [kg P-Eq.] 2.90E-5 4.71E-7 1.05E-8 1.32E-9 2.36E-7 5.22E-7 0.00E+0 -1.42E-5
EP-marine [kg N-Eq.] 1.15E-2 3.56E-5 7.28E-6 1.65E-5 1.78E-5 7.34E-3 0.00E+0 -4.68E-3
EP-terrestrial [mol N-Eq.] 1.21E-1 4.16E-4 1.20E-4 1.81E-4 2.08E-4 8.44E-2 0.00E+0 -5.02E-2
POCP [kg NMVOC-Eq.] 3.90E-2 9.27E-5 2.09E-5 4.69E-5 4.64E-5 1.89E-2 0.00E+0 -1.34E-2
ADPE [kg Sb-Eq.] 8.29E-6 6.80E-9 8.60E-10 1.96E-10 3.40E-9 5.24E-8 0.00E+0 -1.68E-6
ADPF [MJ] 2.41E+2 1.30E+0 7.91E-2 1.01E-1 6.51E-1 6.92E+0 0.00E+0 -1.86E+2
[m³ world-Eq
WDP 1.46E+0 2.11E-3 2.08E-2 1.30E-5 1.05E-3 2.51E+0 0.00E+0 -1.00E+0
deprived]
GWP = Global warming potential; ODP = Depletion potential of the stratospheric ozone layer; AP = Acidification potential of land and water; EP =
Caption Eutrophication potential; POCP = Formation potential of tropospheric ozone photochemical oxidants; ADPE = Abiotic depletion potential for non-
fossil resources; ADPF = Abiotic depletion potential for fossil resources; WDP = Water (user) deprivation potential
RESULTS OF THE LCA - INDICATORS TO DESCRIBE RESOURCE USE according to EN 15804+A2: 1 m2
100/12,5 mm thickness
Indicator Unit A1-A3 A4 A5 C1 C2 C3 C4 D
PERE [MJ] 4.11E+1 7.56E-2 1.53E-2 2.96E-4 3.78E-2 9.20E-1 0.00E+0 -3.78E+1
PERM [MJ] 0.00E+0 0.00E+0 0.00E+0 0.00E+0 0.00E+0 0.00E+0 0.00E+0 0.00E+0
PERT [MJ] 4.11E+1 7.56E-2 1.53E-2 2.96E-4 3.78E-2 9.20E-1 0.00E+0 -3.78E+1
PENRE [MJ] 1.31E+2 1.30E+0 7.92E-2 1.01E-1 6.51E-1 1.17E+2 0.00E+0 -1.86E+2
PENRM [MJ] 1.10E+2 0.00E+0 0.00E+0 0.00E+0 0.00E+0 -1.10E+2 0.00E+0 0.00E+0
PENRT [MJ] 2.41E+2 1.30E+0 7.92E-2 1.01E-1 6.51E-1 6.92E+0 0.00E+0 -1.86E+2
SM [kg] 0.00E+0 0.00E+0 0.00E+0 0.00E+0 0.00E+0 0.00E+0 0.00E+0 0.00E+0
RSF [MJ] 0.00E+0 0.00E+0 0.00E+0 0.00E+0 0.00E+0 0.00E+0 0.00E+0 0.00E+0
NRSF [MJ] 0.00E+0 0.00E+0 0.00E+0 0.00E+0 0.00E+0 0.00E+0 0.00E+0 0.00E+0
FW [m³] 6.57E-2 1.28E-4 4.94E-4 5.47E-7 6.39E-5 5.93E-2 0.00E+0 -4.45E-2
PERE = Use of renewable primary energy excluding renewable primary energy resources used as raw materials; PERM = Use of
renewable primary energy resources used as raw materials; PERT = Total use of renewable primary energy resources; PENRE = Use of
non-renewable primary energy excluding non-renewable primary energy resources used as raw materials; PENRM = Use of non-
Caption
renewable primary energy resources used as raw materials; PENRT = Total use of non-renewable primary energy resources; SM = Use
of secondary material; RSF = Use of renewable secondary fuels; NRSF = Use of non-renewable secondary fuels; FW = Use of net fresh
water
RESULTS OF THE LCA – WASTE CATEGORIES AND OUTPUT FLOWS according to EN 15804+A2:
1 m2 100/12,5 mm thickness
Indicator Unit A1-A3 A4 A5 C1 C2 C3 C4 D
HWD [kg] 8.49E-5 7.28E-8 3.71E-10 1.07E-11 3.64E-8 4.40E-9 0.00E+0 -7.67E-8
NHWD [kg] 8.40E-1 1.06E-4 1.93E-2 6.02E-7 5.29E-5 1.29E-1 0.00E+0 -8.06E-2
RWD [kg] 3.61E-3 1.77E-6 3.64E-6 1.16E-7 8.84E-7 3.11E-4 0.00E+0 -1.51E-2
CRU [kg] 0.00E+0 0.00E+0 0.00E+0 0.00E+0 0.00E+0 0.00E+0 0.00E+0 0.00E+0
MFR [kg] 0.00E+0 0.00E+0 0.00E+0 0.00E+0 0.00E+0 0.00E+0 0.00E+0 0.00E+0
MER [kg] 0.00E+0 0.00E+0 7.99E-2 0.00E+0 0.00E+0 1.16E+1 0.00E+0 0.00E+0
EEE [MJ] 0.00E+0 0.00E+0 4.43E-1 0.00E+0 0.00E+0 4.43E+1 0.00E+0 0.00E+0
EET [MJ] 0.00E+0 0.00E+0 7.98E-1 0.00E+0 0.00E+0 7.92E+1 0.00E+0 0.00E+0
HWD = Hazardous waste disposed; NHWD = Non-hazardous waste disposed; RWD = Radioactive waste disposed; CRU = Components
Caption for re-use; MFR = Materials for recycling; MER = Materials for energy recovery; EEE = Exported electrical energy; EEE = Exported
thermal energy
RESULTS OF THE LCA – additional impact categories according to EN 15804+A2-optional:
1 m2 100/12,5 mm thickness
Indicator Unit A1-A3 A4 A5 C1 C2 C3 C4 D
[Disease
PM 6.47E-7 6.64E-10 3.77E-10 3.96E-10 3.32E-10 4.36E-8 0.00E+0 -1.72E-7
Incidence]
[kBq U235-
IR 5.99E-1 2.59E-4 4.82E-4 1.70E-5 1.29E-4 4.83E-2 0.00E+0 -2.47E+0
Eq.]
ETP-fw [CTUe] 8.57E+1 8.77E-1 5.60E-2 6.81E-2 4.38E-1 2.34E+0 0.00E+0 -4.14E+1
HTP-c [CTUh] 9.66E-9 1.76E-11 4.28E-12 1.16E-12 8.79E-12 3.96E-10 0.00E+0 -7.60E-9
HTP-nc [CTUh] 1.53E-7 7.07E-10 3.14E-10 4.04E-11 3.54E-10 4.61E-9 0.00E+0 -3.82E-8
SQP [-] 1.82E+1 5.87E-1 1.99E-2 2.64E-4 2.94E-1 1.36E+0 0.00E+0 -2.81E+1
PM = Potential incidence of disease due to PM emissions; IR = Potential Human exposure efficiency relative to U235; ETP-fw = Potential
Caption comparative Toxic Unit for ecosystems; HTP-c = Potential comparative Toxic Unit for humans (cancerogenic); HTP-nc = Potential
comparative Toxic Unit for humans (not cancerogenic); SQP = Potential soil quality index
Disclaimer 1 – for the indicator IR
This impact category deals mainly with the eventual impact of low dose ionizing radiation on human health of the
nuclear fuel cycle. It does not consider effects due to possible nuclear accidents, occupational exposure nor due
to radioactive waste disposal in underground facilities. Potential ionizing radiation from the soil, from radon and
from some construction materials is also not measured by this indicator.
Disclaimer 2 – for the indicators ADPE, ADPF, WDP, ETP-fw, HTP-c, HTP-nc, SQP
The results of this environmental impact indicator shall be used with care as the uncertainties on these results are
high or as there is limited experienced with the indicator.
References
EN 13166 2019
EN 13166:2012+A2:2016: Thermal insulation products
for buildings. Factory made phenolic foam (PF) IBU 2016
products. Specification IBU (2016): General Programme Instructions for the
Preparation of EPDs at the Institut Bauen und Umwelt
EN 13950 e.V., Version 1.1 Institut Bauen und Umwelt e.V.,
EN 13950:2014: Gypsum board thermal/acoustic Berlin, www.ibu-epd.de
insulation composite panels - Definitions, requirements
and test methods ISO 14025
EN ISO 14025:2011-10 - Environmental labels and
EN 15804+A2 declarations — Type III environmental declarations —
EN15804/A2: Sustainability of construction works - Principles and procedures
Environmental product declarations - Core rules for the
product category of construction products, 2019 LCA-tool
Kingspan LCA tool, version 1.0. IBU-KSI-202001-LT1-
BPR EN.
Regulation (EU) No 528/2012 of the European Developed by Sphera Solutions GmbH (formely
Parliament and of the Council of 22 May 2012 Thinkstep GmbH)
concerning the making available on the market and
use of biocidal products PCR Version 1.7, Part A
Institut Bauen und Umwelt e.V., Berlin (pub.): Product
CPR Category Rules for Building-Related Products and
Regulation (EU) No. 305/2011 of the European services, Part A: Calculation Rules for the Life Cycle
Parliament and of the Council of 9 March 2011 laying Assessment and Requirements on the Project Report ,
down hamonised condition for the marketing of March 2018
construction products and repealing Council Directive
89/106/EC PCR 2017, Part B
Institut Bauen und Umwelt e.V., Berlin (pub.): Product
GaBi ts Category Rules for Construction Products from the
thinkstep AG: Leinfelden-Echterdingen GaBi Software- range of Environmental Product Declarations of Institut
System and Database for Life Cycle Engineering 1992- Bauen und Umwelt (IBU), Part B: Requirements on the
6 Environmental Product Declaration Kingspan Insulation B.V. – Kooltherm® K17
EPD for insulating materials made of foam
plastics.June 2017 Renewable Energy Certificate
Towarowa Gielda Energii S.A.: Guarantees of origin
REACH Document ID: RGP_ACTBV_2019-12-31_0720
Regulation (EC) No 1907/2006 of the European
Parliament and of the Council on the Registration,
Evaluation, Authorisation and Restriction of Chemicals
(REACH)
https://echa.europa.eu/candidate-list-table; accessed
19th of January 2021, 211 substances listed.
7 Environmental Product Declaration Kingspan Insulation B.V. – Kooltherm® K17
Publisher
Institut Bauen und Umwelt e.V. Tel +49 (0)30 3087748- 0
Panoramastr. 1 Fax +49 (0)30 3087748- 29
10178 Berlin Mail info@ibu-epd.com
Germany Web www.ibu-epd.com
Programme holder
Institut Bauen und Umwelt e.V. Tel +49 (0)30 - 3087748- 0
Panoramastr 1 Fax +49 (0)30 – 3087748 - 29
10178 Berlin Mail info@ibu-epd.com
Germany Web www.ibu-epd.com
Author of the Life Cycle
Assessment Tel +31 (0) 543 543 210
Kingspan Insulation B.V. Fax +31 (0) 344 675 251
Lingewei 8 Mail info@kingspaninsulation.nl
4004LL Tiel Web www.kingspan.com
Netherlands
Owner of the Declaration
Kingspan Insulation B.V. Tel +31 (0) 543 543 210
Lingewei 8 Fax +31 (0) 344 675 251
4004LL Tiel Mail info@kingspaninsulation.nl
Netherlands Web www.kingspan.com
