ENVIRONMENTAL PRODUCT DECLARATION
as per ISO 14025 and EN 15804+A1
Owner of the Declaration Bentzon Carpets ApS
Programme holder Institut Bauen und Umwelt e.V. (IBU)
Publisher Institut Bauen und Umwelt e.V. (IBU)
Declaration number EPD-BTZ-20210007-CCD1-EN
Issue date 24.11.2020
Valid to 23.11.2025
Woven carpet tiles,
pile material polyamide 6.6, max. total pile weight 1500 g/m2
continuous dyeing method, felt backing made of recycled
material
Bentzon Carpets
www.ibu-epd.com | https://epd-online.com
Umwelt Produktdeklaration Name des Herstellers – Name des Produkts
General Information
Bentzon Carpets Woven carpet tiles, pile material
polyamide 6.6, max. total pile weight
1500 g/m2, continuous dyeing method,
felt backing made of recycled material
Programme holder Owner of the declaration
IBU – Institut Bauen und Umwelt e.V. Bentzon Carpets ApS
Panoramastr. 1 Fabrikvej 15, Røjle
10178 Berlin 5500 Middelfart
Germany Denmark
Declaration number Declared product / declared unit
EPD-BTZ-20210007-CCD1-EN 1 m² woven carpet tiles with a pile material of
polyamide 6.6
This declaration is based on the product Scope:
category rules: The manufacturer declaration applies to a group of
Floor coverings, 02/2018 similar products with a maximum total pile weight of
(PCR checked and approved by the SVR) 1500 g/m². The products are manufactured externally
in Denmark.
Issue date LCA results for products with a maximum total pile
weight of 400 g/m2 can be taken from the
24.11.2020
corresponding tables of the annexe. Specific data for
every product within the declared group of products in
Valid to
relation to its total pile weight can be calculated by
23.11.2025 using equation 1 given in the annexe (see annexe
chapter: 'General Information on the annexe').
It is only valid in conjunction with a valid GUT-PRODIS
license of the product.
The owner of the declaration shall be liable for the
underlying information and evidence; the IBU shall not
be liable with respect to manufacturer information, life
cycle assessment data and evidences.
The EPD was created according to the specifications
of EN 15804+A1. In the following, the standard will be
simplified as EN 15804.
Verification
The standard EN 15804 serves as the core PCR
Independent verification of the declaration and data
according to ISO 14025:2010
Dipl. Ing. Hans Peters internally x externally
(chairman of Institut Bauen und Umwelt e.V.)
Dr. Alexander Röder Angela Schindler
(Managing Director Institut Bauen und Umwelt e.V.)) (Independent verifier)
Product
Information about the enterprise produced of the latest developed generations in
Bentzon Carpets manufacture flat woven carpets for polyamide or in 80/20 wool/polyamide.
domestic and contract use, a big part of which is Bentzon Carpets has also established a strong position
exported, primarily to Europe. Bentzon Carpets was on the contract market, where the carpets are installed
established in 1976. Concentrating on quality and an in high traffic areas such as shops, offices, cinemas,
exceptional product differentiation we have created airports, libraries, hotels and means of transport, for
one of the leading productions of exclusive woven example trains. The range of colours and patterns is
carpets, retaining traditional weaving methods. Today, large and we concentrate on manufacturing products
however, the carpets are manufactured on advanced after a Scandinavian minimalistic design. These
high-technology looms ensuring a uniform production products are characterised by a long lasting quality
with the possibility of many different structures. A large and easy maintenance.
part of our domestic products are made of pure new
wool of the best quality, while the contract products are
2 Environmental Product Declaration Bentzon Carpets – Woven carpet tiles, pile material PA 6.6, max. total pile weight
1500 g/m², continuous dyeing method, recycled felt backing
Product description/Product definition
Woven carpet tiles with a pile material made of Performance data of the product in accordance with
polyamide 6.6 with an admixture of polyester and a felt the declaration of performance with respect to its
backing made of 100% recycled polyester. essential characteristics according to EN 14041.
The carpet is coloured by a continuous dyeing method. Additional product properties in accordance with EN
The minimum recycled content out of total weight is 1307 can be found on the Product Information System
10% with a total pile weight of 1500 g/m2. PRODIS using the PRODIS registration number of the
The calculations refer to a total pile weight of maximum product (www.pro-dis.info) or on the manufacturer's
1500 g/m2. technical information section (www.bentzon.dk).
LCA results for products with a maximum total pile
weight of 400 g/m2 can be taken from the Base materials/Ancillary materials
corresponding tables of the annexe.
Results for specific products with any other total pile Name Value Unit
weight can be calculated by using equation 1 given in Polyamide 6.6 39.1 %
the annexe (see annexe chapter: 'General Information Polyester 21.1 %
on the annexe'). Mineral filler 4.9 %
For the placing on the market of the product in the Aluminium hydroxide 19.1 %
European Union/European Free Trade Association Polymer dispersion (solid content) 15.4 %
(EU/EFTA) (with the exception of Switzerland) Additives 0.4 %
Regulation (EU) No. 305/2011 Construction Product
Regulation (CPR) applies. The product needs a The products are registered in the GUT-PRODIS
Declaration of Performance (DoP) taking into Information System. The PRODIS system ensures the
consideration EN 14041, Resilient, textile and laminate compliance with limitations of various chemicals and
floor coverings - Essential characteristics, May 2018, Volatile Organic Compound (VOC)-emissions and a
and the CE-marking. The DoP of the product can be ban on the use of all substances that are listed as
found on the manufacturer's technical information 'Substances of Very High Concern' (SVHC) under
section. For the application and use of the product the REACH.
respective national provisions apply. This product contains substances listed in the ECHA
candidate list (16.01.2020) exceeding 0.1 percentage
Application by mass: no
According to the use class as defined in EN 1307 the
products can be used in all professional areas which Reference service life
require class 33 or less. A calculation of the reference service life according to
ISO 15686 is not possible.
The service life of textile floor coverings strongly
depends on the correct installation taking into account
the declared use classification and the adherence to
cleaning and maintenance instructions.
Technical Data A minimum service life of 10 years can be assumed,
technical service life can be considerably longer.
The performance data listed in the DoP apply.
Name Value Unit
Product Form Tiles of various dimensions -
Type of manufacture Woven loop pile carpet -
Polyamide 6.6 with an
Yarn type -
admixture of polyester
Colouration Continuous dyed
Felt backing made of 100%
Secondary backing -
recycled polyester
Total pile weight max. 1500 g/m²
Total carpet weight max. 3530 g/m2
LCA: Calculation rules
Declared Unit System boundary
Type of EPD: Cradle-to-grave
Name Value Unit
Declared unit 1 m2 System boundaries of modules A, B, C, D:
Conversion factor to 1 kg 0 . 2 8 - Modules C3, C4 and D are indicated separately for
Mass reference 3.53 kg/m² three end-of-life scenarios:
The declared unit refers to 1 m2 produced textile floor 1 - landfill disposal
covering. Output of module A5 'Assembly' is 1 m2 2 - municipal waste incineration
installed textile floor covering. 3 - recovery in a cement plant
3 Environmental Product Declaration Bentzon Carpets – Woven carpet tiles, pile material PA 6.6, max. total pile weight
1500 g/m², continuous dyeing method, recycled felt backing
A1-A3 Production: B3 - B7:
Energy supply and production of the basic material, The modules are not relevant and therefore not
processing of secondary material, auxiliary material, declared.
transport of the material to the manufacturing site,
emissions, waste water treatment, packaging material C1 De-construction:
and waste processing up to the landfill disposal of The floor covering is de-constructed manually and no
residual waste (except radioactive waste). Benefits for additional environmental impact is caused.
generated electricity and steam due to the incineration
of production waste are aggregated. C2 Transport:
Biogenic carbon that is stored in renewable material Transport of the carpet waste to a landfill, to the
(packaging paper) is taken into account as well as the municipal waste incineration plant (MWI) or to the
associated carbon dioxide uptake from the air from waste collection facility for recycling.
which this biogenic carbon comes.
C3 Waste processing:
A4 Transport: C3-1: Landfill disposal needs no waste processing.
Transport of the packed textile floor covering C3-2: Impact from waste incineration (plant with
from factory gate to the place of installation. R1>0.6), generated electricity and steam are listed in
the result table as exported energy.
A5 Installation: C3-3: Collection of the carpet waste, waste processing
Installation of the textile floor covering, processing of (granulating).
installation waste and packaging waste up to the
landfill disposal of residual waste (except radioactive C4 Disposal
waste), the production of the amount of carpet that C4-1: Impact from landfill disposal,
occurs as installation waste including its transport to C4-2: The carpet waste leaves the system in
the place of installation. module C3-2,
Generated electricity and steam due to the incineration C4-3: The pre-processed carpet waste leaves the
of waste are listed in the result table as exported system in module C3-3.
energy.
Biogenic carbon that is stored in renewable materials D Recycling potential:
in packaging paper is released as carbon dioxide Calculated benefits result from materials exclusive
emissions into the air at the end of life in module A5. secondary materials (net materials).
Preparation of the floor and auxiliary materials D-A5: Benefits for generated energy due
(adhesives, fixing agents, PET connectors) are beyond to incineration of packaging and installation waste
the system boundaries and not taken into account. (incineration plant with R1 > 0.6),
D-1: Benefits for generated energy due to landfill
B1 Use: disposal of carpet waste at the end-of-life,
Indoor emissions during the use stage. After the first D-2: Benefits for generated energy due to incineration
year, no product related Volatile Organic Compound of carpet waste at the end-of-life (incineration plant
(VOC) emissions are relevant due to known VOC with R1 > 0.6),
decay curves of the product. D-3: Benefits for saved fossil energy and saved
inorganic material due to recovery of the carpet in a
B2 Maintenance: cement plant at the end-of-life, transport from the
Cleaning of the textile floor covering for a period of 1 reprocessing plant to the cement kiln.
year:
Vacuum cleaning – electricity supply Comparability
Wet cleaning – electricity, water consumption, Basically, a comparison or an evaluation of EPD data
production of the cleaning agent, waste water is only possible if all the data sets to be compared
treatment. were created according to EN 15804 and the building
The declared values in this module have to be context, respectively the product-specific
multiplied by the assumed service life of the floor characteristics of performance, are taken into account.
covering in the building in question.
Background data are taken from the GaBi database
2020, service pack 40. Remaining data gaps are
covered by the ecoinvent 3.6 database, 2019.
LCA: Scenarios and additional technical information
The following information refer to the declared modules Installation in the building (A5)
and are the basis for calculations or can be used for Name Value Unit
further calculations. The indicated values refer to the Material loss 0.11 kg
declared functional unit of all products with a max. total Polyethene packaging waste and installation waste are
pile weight of 1500 g/m2. considered to be incinerated in a municipal waste
incineration plant. Cardboard packaging waste is going
Transport to the construction site (A4) to be recycled.
Name Value Unit Preparation of the floor and auxiliaries (adhesives,
Litres of fuel (truck, EURO 0-6 mix) 0.0083 l/100km fixing agents, PET connectors etc.) are not taken into
Transport distance 700 km account.
Capacity utilisation (including empty
85 %
runs)
4 Environmental Product Declaration Bentzon Carpets – Woven carpet tiles, pile material PA 6.6, max. total pile weight
1500 g/m², continuous dyeing method, recycled felt backing
Maintenance (B2)
The values for cleaning refer to 1 m2 floor covering
used in commercial areas per year.
Depending on the application based on ISO 10874, the
technical service life recommended by the
manufacturer and the anticipated strain on the floor by
customers, the case-specific useful life can be
established. Based on this useful life the effects of
module B2 need to be calculated in order to obtain the
overall environmental impacts.
Name Value Unit
Maintenance cycle (wet cleaning) 1.5 1/year
Maintenance cycle (vacuum cleaning) 208 1/year
Water consumption (wet cleaning) 0.004 m3
Cleaning agent (wet cleaning) 0.09 kg
Electricity consumption 0.314 kWh
Further information on cleaning and maintenance see
www.bentzon.dk
End of Life (C1-C4)
Three different end-of-life scenarios are declared and
the results are indicated separately in module C.
Each scenario is calculated as a 100% scenario.
Scenario 1: 100% landfill disposal
Scenario 2: 100% municipal waste incineration (MWI)
with R1>0.6
Scenario 3: 100% recycling in the cement industry
If combinations of these scenarios have to be
calculated this should be done according to the
following scheme:
EOL-impact = x% impact (Scenario 1)
+ y% impact (Scenario 2)
+ z% impact (Scenario 3)
with x% + y% + z% = 100%
Name Value Unit
Collected as mixed construction waste
3.53 kg
(scenario 1 and 2)
Collected separately (scenario 3) 3.53 kg
Landfilling (scenario 1) 3.53 kg
Energy recovery (scenario 2) 3.53 kg
Energy recovery (scenario 3) 2,68 kg
Recycling (scenario 3) 0.85 kg
Reuse, recovery and/or recycling potentials (D),
relevant scenario information
Recovery or recycling potentials due to the three end-
of-life scenarios (module C) are indicated separately.
Recycling in the cement industry (scenario 3)
VDZ e.V.
The organic material of the carpet is used as an
alternative fuel in a cement kiln. It mainly substitutes
for lignite (64.5%), hard coal (26.5%) and petrol coke
(9.0%).
The inorganic material is substantially integrated into
the cement clinker and substitutes for original material
input.
5 Environmental Product Declaration Bentzon Carpets – Woven carpet tiles, pile material PA 6.6, max. total pile weight
1500 g/m², continuous dyeing method, recycled felt backing
LCA: Results
The LCA results refer to all declared products with a maximum total pile weight of 1500 g/m2.
LCA results for products with a maximum total pile weight of 400 g/m2 can be taken from the corresponding tables
of the annexe. Results for specific products with any other total pile weight can be calculated by using equation 1
given in the annexe (see annexe chapter: 'General Information on the annexe').
The declared result figures in module B2 have to be multiplied by the assumed service life (in years) of the floor
covering in the building under consideration.
Information on un-declared modules: Modules B6, B7, C1, C3/1, C4/2 and C4/3 cause no additional impact (see
chapter "LCA: Calculation rules" in this document) and are therefore marked as 'modules not declared' (MND).
Module C2 represents the transport for scenarios 1, 2 and 3. Column D represents module D/A5. The calculations
are based on the CML characterization factors (version January 2016).
DESCRIPTION OF THE SYSTEM BOUNDARY (X = INCLUDED IN LCA; MND = MODULE NOT DECLARED;
MNR = MODULE NOT RELEVANT)
BENEFITS AND
CONSTRUCTI LOADS
PRODUCT STAGE ON PROCESS USE STAGE END OF LIFE STAGE BEYOND THE
STAGE SYSTEM
BOUNDARIES
6 Environmental Product Declaration Bentzon Carpets – Woven carpet tiles, pile material PA 6.6, max. total pile weight
1500 g/m², continuous dyeing method, recycled felt backing
lairetam
waR
ylppus tropsnarT
gnirutcafunaM
eht
morf
tropsnarT
etis
eht
ot
etag
ylbmessA esU
ecnanetniaM
riapeR
tnemecalpeR tnemhsibrufeR
ygrene
lanoitarepO esu
retaw
lanoitarepO esu
noitcurtsnoc-eD
noitilomed tropsnarT
gnissecorp
etsaW
lasopsiD -esueR -yrevoceR -gnilcyceR laitnetop
A1 A2 A3 A4 A5 B1 B2 B3 B4 B5 B6 B7 C1 C2 C3 C4 D
X X X X X X X MNR MNR MNR MND MND MND X X X X
RESULTS OF THE LCA - ENVIRONMENTAL IMPACT according to EN 15804+A1: 1 m² floor covering
Parameter Unit A1-A3 A4 A5 B1 B2 C2 C3/2 C3/3 C4/1 D D/1 D/2 D/3
GWP [kg CO2-Eq.] 1.86E+1 2.11E-1 7.72E-1 0.00E+0 2.92E-1 1.17E-2 6.67E+0 1.94E-2 2.37E-1 -7.76E-2 0.00E+0-2.50E+0-6.08E-1
-1.10E- -3.54E- -3.42E-
ODP [kg CFC11-Eq.] 2.03E-9 3.47E-176.10E-110.00E+0 1.21E-8 1.92E-181.46E-155.79E-167.72E-16 0.00E+0
15 14 15
AP [kg SO2-Eq.] 2.42E-2 8.90E-4 8.79E-4 0.00E+0 1.16E-3 4.93E-5 4.12E-3 4.06E-5 6.46E-4 -9.80E-5 0.00E+0 -3.15E-3 -2.28E-3
EP [kg (PO4)3--Eq.] 4.73E-3 2.24E-4 1.81E-4 0.00E+0 3.17E-4 1.24E-5 1.06E-3 4.50E-6 6.75E-4 -1.22E-5 0.00E+0 -3.92E-4 -2.66E-4
POCP [kg ethene-Eq.] 2.98E-3 -3.75E-4 8.48E-5 6.29E-5 1.48E-4 -2.08E-5 2.54E-4 2.89E-6 7.29E-5 -8.93E-6 0.00E+0 -2.87E-4 -2.79E-4
ADPE [kg Sb-Eq.] 8.28E-6 1.78E-8 2.52E-7 0.00E+0 4.43E-6 9.87E-10 9.81E-8 6.48E-9 4.61E-8 -1.45E-8 0.00E+0 -4.67E-7 -3.89E-7
ADPF [MJ] 3.53E+2 2.88E+0 1.07E+1 0.00E+0 6.76E+0 1.59E-1 2.37E+0 2.15E-1 3.55E+0-1.09E+00.00E+0-3.50E+1-6.69E+1
GWP = Global warming potential; ODP = Depletion potential of the stratospheric ozone layer; AP = Acidification potential of land and water; EP =
Caption Eutrophication potential; POCP = Formation potential of tropospheric ozone photochemical oxidants; ADPE = Abiotic depletion potential for non-
fossil resources; ADPF = Abiotic depletion potential for fossil resources
RESULTS OF THE LCA - INDICATORS TO DESCRIBE RESOURCE USE according to EN 15804+A1: 1 m²
floor covering
Parameter Unit A1-A3 A4 A5 B1 B2 C2 C3/2 C3/3 C4/1 D D/1 D/2 D/3
PERE [MJ] 3.77E+1 1.62E-1 1.48E+0 0.00E+0 1.20E+0 8.96E-3 3.41E-1 1.54E-1 2.57E-1 -2.93E-1 0.00E+0 -9.42E+0 -7.88E-1
PERM [MJ] 3.22E-1 0.00E+0 -3.22E-1 0.00E+0 0.00E+0 0.00E+0 0.00E+0 0.00E+0 0.00E+0 0.00E+0 0.00E+0 0.00E+0 0.00E+0
PERT [MJ] 3.80E+1 1.62E-1 1.16E+0 0.00E+0 1.20E+0 8.96E-3 3.41E-1 1.54E-1 2.57E-1 -2.93E-1 0.00E+0 -9.42E+0 -7.88E-1
PENRE [MJ] 2.99E+2 2.89E+0 1.14E+1 0.00E+0 7.86E+0 1.60E-1 7.52E+1 7.30E+1 3.66E+0 -1.34E+0 0.00E+0 -4.31E+1 -6.75E+1
PENRM [MJ] 7.27E+1 0.00E+0 -7.56E-2 0.00E+0 0.00E+0 0.00E+0 -7.27E+1 -7.27E+1 0.00E+0 0.00E+0 0.00E+0 0.00E+0 0.00E+0
PENRT [MJ] 3.72E+2 2.89E+0 1.13E+1 0.00E+0 7.86E+0 1.60E-1 2.59E+0 3.47E-1 3.66E+0 -1.34E+0 0.00E+0 -4.31E+1 -6.75E+1
SM [kg] 4.59E-1 0.00E+0 1.38E-2 0.00E+0 0.00E+0 0.00E+0 0.00E+0 0.00E+0 0.00E+0 0.00E+0 0.00E+0 0.00E+0 8.47E-1
RSF [MJ] 0.00E+0 0.00E+0 0.00E+0 0.00E+0 0.00E+0 0.00E+0 0.00E+0 0.00E+0 0.00E+0 0.00E+0 0.00E+0 0.00E+0 0.00E+0
NRSF [MJ] 0.00E+0 0.00E+0 0.00E+0 0.00E+0 0.00E+0 0.00E+0 0.00E+0 0.00E+0 0.00E+0 0.00E+0 0.00E+0 0.00E+0 7.27E+1
FW [m³] 6.63E-2 1.88E-4 2.52E-3 0.00E+0 4.27E-3 1.04E-5 1.72E-2 1.78E-4 4.50E-5 -3.40E-4 0.00E+0 -1.09E-2 -6.07E-3
PERE = Use of renewable primary energy excluding renewable primary energy resources used as raw materials; PERM = Use of
renewable primary energy resources used as raw materials; PERT = Total use of renewable primary energy resources; PENRE = Use of
non-renewable primary energy excluding non-renewable primary energy resources used as raw materials; PENRM = Use of non-
Caption
renewable primary energy resources used as raw materials; PENRT = Total use of non-renewable primary energy resources; SM = Use
of secondary material; RSF = Use of renewable secondary fuels; NRSF = Use of non-renewable secondary fuels; FW = Use of net fresh
water
RESULTS OF THE LCA – WASTE CATEGORIES AND OUTPUT FLOWS according to EN 15804+A1:
1 m² floor covering
Parameter Unit A1-A3 A4 A5 B1 B2 C2 C3/2 C3/3 C4/1 D D/1 D/2 D/3
HWD [kg] 4.80E-7 1.34E-7 1.89E-8 0.00E+0 9.63E-10 7.43E-9 5.93E-9 1.44E-10 1.34E-8 -5.34E-10 0.00E+0 -1.72E-8 2.61E-9
NHWD [kg] 5.14E-1 4.42E-4 2.81E-2 0.00E+0 5.63E-3 2.44E-5 4.22E-1 2.46E-4 3.52E+0 -6.20E-4 0.00E+0 -1.99E-2 -3.23E-1
RWD [kg] 7.54E-3 3.57E-6 2.29E-4 0.00E+0 3.38E-4 1.98E-7 8.99E-5 5.27E-5 4.42E-5 -1.00E-4 0.00E+0 -3.22E-3 -2.09E-4
CRU [kg] 0.00E+0 0.00E+0 0.00E+0 0.00E+0 0.00E+0 0.00E+0 0.00E+0 0.00E+0 0.00E+0 0.00E+0 0.00E+0 0.00E+0 0.00E+0
MFR [kg] 8.56E-2 0.00E+0 1.15E-1 0.00E+0 0.00E+0 0.00E+0 0.00E+0 8.47E-1 0.00E+0 0.00E+0 0.00E+0 0.00E+0 0.00E+0
MER [kg] 0.00E+0 0.00E+0 0.00E+0 0.00E+0 0.00E+0 0.00E+0 0.00E+0 2.68E+0 0.00E+0 0.00E+0 0.00E+0 0.00E+0 0.00E+0
EEE [MJ] 0.00E+0 0.00E+0 3.69E-1 0.00E+0 0.00E+0 0.00E+0 1.19E+1 0.00E+0 0.00E+0 0.00E+0 0.00E+0 0.00E+0 0.00E+0
EET [MJ] 0.00E+0 0.00E+0 6.65E-1 0.00E+0 0.00E+0 0.00E+0 2.15E+1 0.00E+0 0.00E+0 0.00E+0 0.00E+0 0.00E+0 0.00E+0
HWD = Hazardous waste disposed; NHWD = Non-hazardous waste disposed; RWD = Radioactive waste disposed; CRU = Components
Caption for re-use; MFR = Materials for recycling; MER = Materials for energy recovery; EEE = Exported electrical energy; EEE = Exported
thermal energy
References
EN 1307 ECHA candidate list
DIN EN 1307: 2014+A1:2016: Textile floor coverings - Candidate List of substances of very high concern
Classification (SVHCs) for authorisation, 16.01.2020, European
Chemicals Agency (ECHA), Helsinki, Finland
EN 13501-1
DIN EN 13501-1:2010-01: Fire classification of ecoinvent 3.6
construction products and building elements - Part 1: ecoinvent, Zurich, Switzerland, database version 3.6,
Classification using data from reaction to fire tests published September 2019
EN 14041 GaBi database 2020
DIN EN 14041: 2018-05: Resilient, textile and laminate GaBi Software-System and Database for Life Cycle
floor coverings - Essential characteristics Engineering, thinkstep AG, Leinfelden-Echterdingen,
service pack 40, 2020
EN 15804
EN 15804:2012-04+A1 2013/, Sustainability of IBU 2016
construction works — Environmental Product IBU (2016): General Programme Instructions for the
Declarations — Core rules for the product category of Preparation of EPDs at the Institut Bauen und Umwelt
construction products e.V., Version 1.1 Institut Bauen und Umwelt e.V.,
Berlin, www.ibu-epd.de
EN 16810
DIN EN 16810: 2017-08: Resilient, textile and laminate PCR Part A
floor coverings – Environmental product declarations – Product Category Rules for Construction Products
Product category rules from the range of Environmental Product Declarations.
Part A: Calculation Rules for the Life Cycle
ISO 10874 Assessment and Requirements on the Background
DIN EN ISO 10874: 2012-04: Resilient, textile and Report, V1.8, Berlin: Institut Bauen und Umwelt e.V.
laminate floor coverings - Classification (IBU), July 2019
ISO 14025 PCR Part B
DIN EN /ISO 14025:2011-10: Environmental labels Product Category Rules for Construction Products
and declarations — Type III environmental from the range of Environmental Product Declarations
declarations — Principles and procedures of Institut Bauen und Umwelt (IBU),
Part B: Requirements on the EPD for floor coverings,
ISO 15686 V1.2, Berlin: Institut Bauen und Umwelt e.V. (IBU),
ISO 15686: Buildings and constructed assets - February 2018
Service life planning
ISO 15686-1: 2011-05: Part 1: General principles and PRODIS
framework Product Information System (PRODIS) of the
ISO 15686-2: 2012-05: Part 2: Service life prediction European Carpet Industry, Gemeinschaft
procedures umweltfreundlicher Teppichboden e.V (GUT) and
ISO 15686-7: 2006-03: Part 7: Performance European Carpet and Rug Association
evaluation for feedback of service life data (ECRA), http://www.pro-dis.info
from practice
ISO 15686-8: 2008-06: Part 8: Reference service life REACH
and service-life estimation Regulation (EC) No 1907/2006 of the European
Parliament and of the Council of 18 December 2006
Regulation (EU) No. 305/2011 concerning the Registration, Evaluation, Authorisation
Regulation No. 305/2011 Construction Products and Restriction of Chemicals (REACH). Last update:
Regulation (CPR) of the European Council and of the 25.03.2014 (Status: 27.06.2018)
European Parliament, April 2011
VDZ e.V.
Association of German Cement Works, Ed. Environ-
CML characterization factors mental Data of the German Cement Industry 2018
Impact assessment characterization factors, Institute of
Environmental Sciences - in Dutch 'Centrum voor
Milieuwetenschappen in Leiden' (CML), Leiden, The
Netherlands
7 Environmental Product Declaration Bentzon Carpets – Woven carpet tiles, pile material PA 6.6, max. total pile weight
1500 g/m², continuous dyeing method, recycled felt backing
Publisher
Institut Bauen und Umwelt e.V. Tel +49 (0)30 3087748- 0
Panoramastr. 1 Fax +49 (0)30 3087748- 29
10178 Berlin Mail info@ibu-epd.com
Germany Web www.ibu-epd.com
Programme holder
Institut Bauen und Umwelt e.V. Tel +49 (0)30 - 3087748- 0
Panoramastr 1 Fax +49 (0)30 – 3087748 - 29
10178 Berlin Mail info@ibu-epd.com
Germany Web www.ibu-epd.com
Author of the Life Cycle
Assessment Tel +49 (0)241 96843 410
Gemeinschaft umweltfreundlicher Fax +49 (0)241 96843 400
Teppichboden (GUT) e.V. Mail mail@gut-ev.de
Schönebergstraße 2 Web www.gut-ev.org
52068 Aachen
Germany
Owner of the Declaration
Bentzon Carpets ApS Tel +45 (0) 64 40 20 00
Fabrikvej 15 Røjle Fax +45 (0) 64 40 24 24
5500 Middelfart Mail info@bentzon.dk
Denmark Web www.bentzon.dk
