ENVIRONMENTAL PRODUCT DECLARATION
as per ISO 14025 and EN 15804+A1
Owner of the Declaration JACKON Insulation GmbH
Programme holder Institut Bauen und Umwelt e.V. (IBU)
Publisher Institut Bauen und Umwelt e.V. (IBU)
Declaration number EPD-JAI-20200164-IBC1-EN
Issue date 16.03.2021
Valid to 15.03.2026
JACKODUR Plus - Extruded Polystyrene (XPS)
with HFO 1234ze
JACKON Insulation GmbH
www.ibu-epd.com | https://epd-online.com
Umwelt Produktdeklaration Name des Herstellers – Name des Produkts
1. General Information
JACKON Insulation GmbH XPS insulation panel JACKODUR Plus
Programme holder Owner of the declaration
IBU – Institut Bauen und Umwelt e.V. JACKON Insulation GmbH
Panoramastr. 1 Carl-Benz-Str. 8
10178 Berlin 33803 Steinhagen
Germany Germany
Declaration number Declared product / declared unit
EPD-JAI-20200164-IBC1-EN JACKODUR Plus (extruded polystyrene foam) boards
produced by JACKON Insulation GmbH. The EPD
applies to 1 m3 XPS board, with an average density of
35,54 kg/m3.
This declaration is based on the product Scope:
category rules: JACKON Insulation as data provider produces the
Insulating materials made of foam plastics, 06.2017 extruded polystyrene foam boards JACKODUR Plus
(PCR checked and approved by the SVR) containing HFO 1234ze as blowing agent. The data
have been provided by one factory in
Arendsee/Germany for the year 2019.
Issue date
16.03.2021
The owner of the declaration shall be liable for the
underlying information and evidence; the IBU shall not
Valid to
be liable with respect to manufacturer information, life
15.03.2026
cycle assessment data and evidences.
The EPD was created according to the specifications
of EN 15804+A1. In the following, the standard will be
simplified as EN 15804.
Verification
The standard EN 15804 serves as the core PCR
Independent verification of the declaration and data
according to ISO 14025:2010
Dipl. Ing. Hans Peters internally x externally
(chairman of Institut Bauen und Umwelt e.V.)
Dr. Alexander Röder Dr. Frank Werner
(Managing Director Institut Bauen und Umwelt e.V.)) (Independent verifier appointed by SVR)
2. Product
2.1 Product description/Product definition consideration EN 13164. Thermal Insulation products
JACKODUR Plus is an extruded polystyrene foam for buildings and the CE-marking. For the application
(XPS) produced according to EN 13164 and available and use the respective national provisions apply.
in board shape with a density range from 30 to 50
kg/m3, 35,54 kg/m3 in average (measured). It has 2.2 Application
specifically low values of thermal conductivity by using The variety of the performance properties of
Hydrofluoroolefins (HFO)1234 ze as blowing agent. JACKODUR Plus make it suitable for use in a large
The boards are also called Super XPS in Scandinavia. number of applications such as: perimeter insulation,
The boards can be delivered in various compressive inverted roof insulation, insulation of pitched roofs,
strength values from 300 to 700 kPa. To meet the floor insulation including insulation of highly loaded
need of various applications the boards are produced industrial floors, insulation of thermal bridges for
with different surfaces: with the extrusion skin, planed, exterior walls, External Thermal Insulation Composite
grooved or with thermal embossing. JACKODUR Plus Systems (ETICS), insulation of cavity walls, agricultural
boards are supplied with different edge treatments building ceiling insulation, prefabricated elements e.g.
such as butt edge, ship-lap and tongue and groove. building sandwich panels, insulation for building
The EPD is related to an unlaminated product only; equipment and industrial installations (pipe sections,
lamination and additional product treatment are not …).
considered.
For the placing on the market of the product in the 2.3 Technical Data
European Union/European Free Trade Association Acoustic properties are not relevant for JACKODUR
(EU/EFTA) (with the exception of Switzerland) Plus. For fire performance, these products except in
Regulation (EU) No. 305/2011 (CPR) applies. The Scandinavia achieve the fire classification Euroclass E
product needs a declaration of performance taking into according to EN 13501-1.
2 Environmental Product Declaration Jackon Insulation GmbH – XPS Foam Insulation Jackodur plus
Reptrotoxic (CMR) substances in categories 1A or 1B
which are not on the candidate list, exceeding 0.1
Constructional data percentage by mass: no
Name Value Unit Biocide products were added to this construction
Gross density 30 - 50 kg/m3 product or it has been treated with biocide products
Calculation value for thermal (this then concerns a treated product as defined by the
0.025 -
conductivity acc. to EN 12667 and W/(mK) (EU) Ordinance on Biocide Products No. 528/2012):
0.027
EN 13164 Annex C no
Water vapour diffusion resistance
50 - 250 -
factor acc. to EN 12086
Water absorption after diffusion 2.6 Manufacture
3 - 5 Vol.-%
acc. to EN 12088 JACKODUR Plus is produced by a continuous
Deformation under compressive extrusion process using electricity as the main power
load and temperature acc. to EN ≤ 5 % source: polystyrene granules are melted in an extruder
1605 and a blowing agent is injected into the extruder under
Compressive stress or strength at high pressure.
10% deflection acc. to EN 826 300 - 700 kPa The drop in pressure at the exit die causes the
Compressive modulus of elasticity 10000 - polystyrene to foam into a board with homogeneous
acc. to EN 826 40000 kPa and closed-cell structure.
Then the boards’ edges are trimmed, and the product
Tensile strength perpendicular to
100 - 400 kPa is cut to dimensions. The smooth foam skin resulting
faces acc. to EN 1607
from the extrusion process remains on the boards or is
Compressive creep/long-term
removed mechanically for particular board types to
compressive strength acc. to EN < 250 kPa
achieve better adhesive strength in combination with e.
1606
g. concrete, mortar, or construction adhesives. Some
Freeze-thaw resistance acc. to EN
≤ 2 Vol.-% boards receive special surface patterns or grooves.
12091
JACKODUR Plus foams off-grade material or scrap
Dimensional stability acc. to EN
≤ 5 % from production is recycled in the production process
1604
of extruded polystyrene foam XPS.
The manufacturing plant in Arendsee/Germany is
certified according to ISO 9001 and ISO 50001.
Performance data of the product in accordance with
the declaration of performance with respect to its
essential characteristics according to EN
2.7 Environment and health during
13164:2012+A1:2015 Thermal Insulation products for
manufacturing
buildings.
No further health protection measures beyond the
regulated measures for manufacturing firms are
2.4 Delivery status
necessary during all production steps. The
Length: 1000-3000 mm; Width: 600-1500 mm;
manufacturing plant in Arendsee/Germany is certified
Thickness: 20-320 mm.
according to ISO 14001.
2.5 Base materials/Ancillary materials
2.8 Product processing/Installation
JACKODUR Plus is mostly made of polystyrene (90 to
Handling recommendations for JACKODUR Plus can
95% by weight in the final product – CAS 9003-53-6),
be found in product and application literature,
blown with fluorinated olefin (HFO1234ze), carbon
brochures and data sheets provided directly by
dioxide (CAS 124-38-9) and halogen-free co-blowing
suppliers or available from the internet. There are no
agents altogether up to 8.5% by weight in relation to
special instructions required regarding personal
the material input. The blowing agents are partly
precautions and environmental protection during
emitted during the production process.
product handling and installation.
Basic material Mass portion
2.9 Packaging
Polystyrene 90 - 91 %
The polyethylene-based packaging film is recyclable
Blowing agents 8,5 %
and (actually) recycled in those countries having a
HFO 1234ze ~ 70 %
return system.
CO2, and Co-blowing Agents ~ 30 %
Flame retardant 0 - 2 %
Additives (e.g. pigments) < 0,5%
2.10 Condition of use
Water pick-up by capillarity does generally not occur
The brominated flame retardant is used to enable the
with JACKODUR plus due to their closed-cell structure.
foam to meet fire performance standards. Other
The thermal insulation performance of XPS is
additives are used, e. g. colour pigments and
practically not affected by exposure to water or water
processing aids in minor quantity, less than 0.5%.
vapour.
Polystyrene is produced from oil and gas. Therefore it
Usually, maintenance will not be required if the XPS
is linked to the availability of these raw materials.
boards are installed according to handling installation
Polystyrene is transported by road.
requirements (see: Installation description).
This product contains substances listed in the
2.11 Environment and health during use
candidate list of substances of very high concern
JACKODUR Plus is in most applications not in direct
(REACH Regulation, date:15.01.2019) exceeding 0.1
contact with the environment nor with the indoor air.
percentage by mass: no
This product contains other Carcinogenic, Mutagenic,
3 Environmental Product Declaration Jackon Insulation GmbH – XPS Foam Insulation Jackodur plus
2.12 Reference service life 2.14 Re-use phase
A reference service life (RSL) according to ISO 15686 In order to maximize the potential to re-use
cannot be declared. JACKODUR Plus boards, one must avoid that it is
The durability of JACKODUR Plus is normally at least damaged or glued. Instead separation layers between
as long as the lifetime of the building in which it is the insulation and the concrete should be used or
used. mechanical fixation should be applied.
In the inverted roof application JACKODUR Plus is
installed loose laid and therefore can be easily
removed and reused on another roof. For existing
conventional flat-roofs JACKODUR Plus can stay in
2.13 Extraordinary effects place when for example the existing roof construction
is thermally upgraded as a Plus-roof. Recovered
Fire JACKODUR Plus from mechanically fixed applications
JACKODUR Plus except in Scandinavia achieves the can be reused for insulation of basement walls and
fire classification Euroclass E according to EN 13501- foundations.
1. If contact with the external flame stops, neither Due to the high calorific value of polystyrene, energy
further burning nor smouldering can be observed. embedded in JACKODUR Plus can be recovered in
Ignition of the foam can only be observed after longer municipal waste incinerators equipped with energy
small flame exposures. recovery units for steam and electricity generation and
district heating.
Fire performance 2.15 Disposal
Name Value JACKODUR Plus boards that cannot be easily
Building material class E retrieved from the building are usually landfilled. The
material is assigned
Water to the waste category: 17 06 04 insulation materials
Water pick-up by capillarity does generally not occur other than those mentioned in 17 06 01 (insulation
with XPS foams due to their closed-cell structure. The materials containing asbestos) and 17 06 03 (other
thermal insulation performance of JACKODUR Plus is insulation materials consisting of or containing
practically not affected by exposure to water or water dangerous substances) European Waste Catalogue,
vapour. AVV.
Mechanical destruction 2.16 Further information
Not relevant for JACKODUR Plus. Additional information can be found at the web page
www.jackon-insulation.com.
3. LCA: Calculation rules
3.1 Declared Unit 3.2 System boundary
The declared unit is 1 m3 XPS. Type of EPD: cradle-to-gate (A1 - A3) – with options.
Corresponding conversion factors are listed in the The following modules are considered in the Life Cycle
table below. Assessment:
• The raw material supply (A1) comprises the
Declared unit production of polysterene granulate, blowing agents
Name Value Unit and flame retardants.
Declared unit 1 m3 • The transport to manufacturer is considered in
Gross density 35.54 kg/m3 module A2.
Conversion factor to 1 kg 35.54 - • The manufacturing of XPS (A3) comprises the
energy consumption, packaging of the product and
JACKODUR Plus is available in several densities and auxilliaries.
thicknesses. For a product with a density or thickness • Transport to construction site is calculated with 500
different from the reference density of 35.54 kg/m3, the km via truck (A4).
environmental impacts may be calculated using the • Incineration of packaging materials are considered
following equation: in module A5.
• Transport to disposal (EoL) is calculated with 50
km via truck (C2).
• For the End-of-Life stage two different scenarios
are considered in the LCA. One scenario with 100%
landfill (module C4) and one scenario with 100%
incineration (module C3) are calculated. The
Iadap – adapted Life Cycle Impact Assessment LCIA incineration of XPS results in credits for thermal energy
indicator or LCI parameter and power under European boundary conditions (D) -
Iref – LCIA indicator or LCI parameter for reference beyond system boundary.
density of 35.54 kg/m3
ρradap – adapted density 3.3 Estimates and assumptions
ρref – reference density 35.54 kg/m3 The environmental profile of the flame retardant is
dadap – adapted board thickness based on valid estimations, based on literature data,
dref – thickness of reference board 100mm basically Ullmanns.
4 Environmental Product Declaration Jackon Insulation GmbH – XPS Foam Insulation Jackodur plus
3.4 Cut-off criteria done for waste respective recycling materials only.
In the assessment, all available data from the
production process are considered, i.e. all raw Allocation for waste materials:
materials used, utilised electric power consumption Post-industrial XPS waste from extrusion lines is
using best available LCI datasets. directly reused in the process.
The amount of pigments, which underruns a ratio of In the End-of-Life scenario, all applied incineration
0.5 mass-%, is included in the declared mass of processes are displayed via a partial stream
polystyrene. consideration for the combustion process, according to
the specific composition of the incinerated material.
For the waste incineration plant, an R1-value of > 0.6
3.5 Background data is assumed.
Background data is taken from the GaBi software GaBi
ts, see http://documentation.gabi-software.com/. The environmental burden of the incineration of the
Additionally, a life cycle inventory (LCI) of an existing product in the EoL-scenario are assigned to the
study on behalf of Honeywell, covering the impacts of system (C3); resulting potential benefits for thermal
the manufacturing process of HFO1234ze blowing and electrical energy are declared in module D.
agent, has been used. The LCI is based on the Potential benefits are given according to the European
ecoinvent database. The producing Honeywell facility average data for electrical and thermal energy
is located in the US. generated from natural gas.
3.6 Data quality Allocation for upstream data
The foreground data, mainly the raw material and For all refinery products, allocation by mass and net
energy consumption during the production process is calorific value has been applied. The manufacturing
measured data. route of every refinery product is modelled and the
Most of the necessary life cycle inventories are product-specific effort associated with their production
available in GaBi ts. The last update of the database is calculated.
was 2020. For other materials' inventory used in the production
process calculation the most suitable allocation rules
3.7 Period under review are applied. Information on single LCIs is documented
The foreground data collected by JACKON Insulation on http://documentation.gabi-software.com/.
are based on the yearly production amount and
extrapolations of measurements on specific machines 3.9 Comparability
and plants. The production data refer to an average of Basically, a comparison or an evaluation of EPD data
the year 2019 in the JACKON plant is only possible if all the data sets to be compared
Arendsee/Germany. were created according to EN 15804 and the building
context, respectively the product-specific
3.8 Allocation characteristics of performance, are taken into account.
There are no co-products generated during the XPS-
production. Allocations in the foreground system are The used background database is GaBi ts.
4. LCA: Scenarios and additional technical information
The following technical information is a basis for the End of life (C1-C4)
declared modules or can be used for developing For the End of Life stage, two different scenarios are
specific scenarios in the context of a building considered. One scenario with 100% incineration (C3,
assessment if modules are not declared (MND). sc. 1) and one scenario with 100% landfill (C4, sc. 2)
The values refer to the declared unit of 1 m3 XPS. are calculated. The incineration of XPS results in
potential benefits, beyond the system boundary, for
Transport to the building site (A4) thermal energy and electricity under European
Name Value Unit conditions.
Payload of truck 5 t Name Value Unit
Litres of fuel diesel with maximum Collected separately XPS 35.5 kg
0.18 l/100km
load Collected as mixed construction
0 kg
Transport distance 500 km waste
Capacity utilisation (including Reuse 0 kg
20 %
empty runs) Recycling 0 kg
Gross density of products Energy recovery Scenario 1 35.5 kg
35.5 kg/m3
transported Landfilling Scenario 2 35.5 kg
Capacity utilisation volume factor 0.26 - Reuse, recovery and/or recycling potentials (D),
relevant scenario information
Installation phase (Module A5)
Module D includes the potential benefits beyond
Packaging waste treatment has been included as system boundaries of the incineration process C3
incineration of plastics (A5). The incineration of the (incineration of XPS boards). A waste incineration
packaging materials results in benefits, beyond the plant with R1-value > 0.6 is assumed.
system boundary, for thermal energy and electricity
under European conditions (D).
5 Environmental Product Declaration Jackon Insulation GmbH – XPS Foam Insulation Jackodur plus
5. LCA: Results
The following tables display the environmental relevant results according to EN 15804 for 1 m3 XPS board.
The two EoL scenarios are declared in modules C3/1 + D/1 (Sc. 1) and C4/2 + D/2 (Sc. 2). C3/1 represents the
thermal treatment of XPS-boards and C4/2 the landfilling of XPS. Module D/1 includes benefits and loads beyond
the system boundary for the incineration of packaging materials and the burning of the product during its EoL
(scenario 1). Module D/1 includes only benefits and loads beyond the system boundary of the packaging
materials incineration.
DESCRIPTION OF THE SYSTEM BOUNDARY (X = INCLUDED IN LCA; MND = MODULE NOT DECLARED;
MNR = MODULE NOT RELEVANT)
BENEFITS AND
CONSTRUCTI LOADS
PRODUCT STAGE ON PROCESS USE STAGE END OF LIFE STAGE BEYOND THE
STAGE SYSTEM
BOUNDARIES
6 Environmental Product Declaration Jackon Insulation GmbH – XPS Foam Insulation Jackodur plus
lairetam
waR
ylppus tropsnarT
gnirutcafunaM
eht
morf
tropsnarT
etis
eht
ot
etag
ylbmessA esU
ecnanetniaM
riapeR
tnemecalpeR tnemhsibrufeR
ygrene
lanoitarepO esu
retaw
lanoitarepO esu
noitcurtsnoc-eD
noitilomed tropsnarT
gnissecorp
etsaW
lasopsiD -esueR -yrevoceR -gnilcyceR laitnetop
A1 A2 A3 A4 A5 B1 B2 B3 B4 B5 B6 B7 C1 C2 C3 C4 D
X X X X X MND MND MNR MNR MNR MND MND MND X X X X
RESULTS OF THE LCA - ENVIRONMENTAL IMPACT according to EN 15804+A1: 1 m³ Jackodur Plus XPS
board
Parameter Unit A1-A3 A4 A5 C2 C3/1 C4/2 D/1 D/2
GWP [kg CO2-Eq.] 1.21E+2 5.96E+0 7.49E-1 8.83E-1 1.19E+2 2.35E+0 -4.98E+1 -3.83E-1
ODP [kg CFC11-Eq.] 5.02E-6 9.79E-16 2.91E-16 1.45E-16 1.08E-14 7.77E-15 -7.14E-13 -5.46E-15
AP [kg SO2-Eq.] 6.86E-1 1.44E-2 1.74E-4 2.13E-3 6.75E-3 6.50E-3 -6.34E-2 -4.87E-4
EP [kg (PO4)3--Eq.] 3.82E-2 3.50E-3 1.38E-5 5.18E-4 1.44E-3 6.80E-3 -7.89E-3 -6.06E-5
POCP [kg ethene-Eq.] 1.87E-1 -5.09E-3 6.50E-6 -7.54E-4 6.79E-4 7.34E-4 -5.77E-3 -4.43E-5
ADPE [kg Sb-Eq.] 1.94E-4 4.95E-7 5.14E-8 7.33E-8 7.75E-7 4.64E-7 -9.39E-6 -7.20E-8
ADPF [MJ] 3.16E+3 8.12E+1 2.62E-1 1.20E+1 1.18E+1 3.58E+1 -7.01E+2 -5.40E+0
GWP = Global warming potential; ODP = Depletion potential of the stratospheric ozone layer; AP = Acidification potential of land and water; EP =
Caption Eutrophication potential; POCP = Formation potential of tropospheric ozone photochemical oxidants; ADPE = Abiotic depletion potential for non-
fossil resources; ADPF = Abiotic depletion potential for fossil resources
RESULTS OF THE LCA - RESOURCE USE according to EN 15804+A1: 1 m³ Jackodur Plus XPS board
Parameter Unit A1-A3 A4 A5 C2 C3/1 C4/2 D/1 D/2
PERE [MJ] 2.17E+2 4.57E+0 5.94E-2 6.77E-1 2.65E+0 2.59E+0 -1.90E+2 -1.45E+0
PERM [MJ] 0.00E+0 0.00E+0 0.00E+0 0.00E+0 0.00E+0 0.00E+0 0.00E+0 0.00E+0
PERT [MJ] 2.17E+2 4.57E+0 5.94E-2 6.77E-1 2.65E+0 2.59E+0 -1.90E+2 -1.45E+0
PENRE [MJ] 1.86E+3 8.14E+1 1.32E+1 1.21E+1 1.43E+3 3.69E+1 -8.65E+2 -6.65E+0
PENRM [MJ] 1.43E+3 0.00E+0 -1.29E+1 0.00E+0 -1.42E+3 0.00E+0 0.00E+0 0.00E+0
PENRT [MJ] 3.29E+3 8.14E+1 2.92E-1 1.21E+1 1.38E+1 3.69E+1 -8.65E+2 -6.65E+0
SM [kg] 0.00E+0 0.00E+0 0.00E+0 0.00E+0 0.00E+0 0.00E+0 0.00E+0 0.00E+0
RSF [MJ] 0.00E+0 0.00E+0 0.00E+0 0.00E+0 0.00E+0 0.00E+0 0.00E+0 0.00E+0
NRSF [MJ] 0.00E+0 0.00E+0 0.00E+0 0.00E+0 0.00E+0 0.00E+0 0.00E+0 0.00E+0
FW [m³] 2.87E+1 5.29E-3 1.86E-3 7.84E-4 2.28E-1 4.53E-4 -2.20E-1 -1.68E-3
PERE = Use of renewable primary energy excluding renewable primary energy resources used as raw materials; PERM = Use of
renewable primary energy resources used as raw materials; PERT = Total use of renewable primary energy resources; PENRE = Use of
non-renewable primary energy excluding non-renewable primary energy resources used as raw materials; PENRM = Use of non-
Caption
renewable primary energy resources used as raw materials; PENRT = Total use of non-renewable primary energy resources; SM = Use
of secondary material; RSF = Use of renewable secondary fuels; NRSF = Use of non-renewable secondary fuels; FW = Use of net fresh
water
RESULTS OF THE LCA – OUTPUT FLOWS AND WASTE CATEGORIES according to EN 15804+A1:
1 m³ Jackodur Plus XPS board
Parameter Unit A1-A3 A4 A5 C2 C3/1 C4/2 D/1 D/2
HWD [kg] 1.14E-6 3.79E-6 9.88E-10 5.61E-7 1.17E-8 1.35E-7 -3.45E-7 -2.65E-9
NHWD [kg] 7.97E-1 1.25E-2 7.25E-2 1.85E-3 6.84E-1 3.54E+1 -4.01E-1 -3.08E-3
RWD [kg] 3.85E-2 1.01E-4 1.20E-5 1.49E-5 8.03E-4 4.45E-4 -6.49E-2 -4.97E-4
CRU [kg] 0.00E+0 0.00E+0 0.00E+0 0.00E+0 0.00E+0 0.00E+0 0.00E+0 0.00E+0
MFR [kg] 0.00E+0 0.00E+0 0.00E+0 0.00E+0 0.00E+0 0.00E+0 0.00E+0 0.00E+0
MER [kg] 0.00E+0 0.00E+0 0.00E+0 0.00E+0 0.00E+0 0.00E+0 0.00E+0 0.00E+0
EEE [MJ] 0.00E+0 0.00E+0 1.66E+0 0.00E+0 2.16E+2 0.00E+0 0.00E+0 0.00E+0
EET [MJ] 0.00E+0 0.00E+0 3.00E+0 0.00E+0 3.84E+2 0.00E+0 0.00E+0 0.00E+0
HWD = Hazardous waste disposed; NHWD = Non-hazardous waste disposed; RWD = Radioactive waste disposed; CRU = Components
Caption for re-use; MFR = Materials for recycling; MER = Materials for energy recovery; EEE = Exported electrical energy; EEE = Exported
thermal energy
6. LCA: Interpretation
Regarding the production of JACKODUR Plus, related to the provided Life Cycle Inventory (LCI) and
polystyrene dominates the impact categories global the used Ecoinvent background data.
warming potential (GWP), resource depletion fossil
(ADPF) and the corresponding primary energy non- The summer smog potential (POCP) is less related to
renewable (PENRT) with 61%, 77% and 75% raw materials. The direct emissions during production
contribution as compared to the production stage. generate half of the impact in this category (45% from
DME, 55% from HFO).
The direct emissions are comparably marginal Moreover, polystyrene is relevant for the summer
regarding GWP, since CO2 as blowing agent is used smog with 10%, the production of blowing agents with
only in a small amount (0.7% of raw material input) and another 10%.
the co-blowing agent has no influence on GWP from
the scientific perspective. Transport processes and flame retardant production
The mainly used halogenated blowing agent has a low are of low relevance within the considered indicators.
GWP value as well.
Regarding the whole life cycle (LC) with the inclusion
Resource depletion elements (ADPE), acidification of the End of Life scenarios, the results differ strongly
(AP) and ozone depletion potential (ODP) are mainly between these two scenarios: landfill and incineration
driven by the production of blowing agents, primarily with energy recovery. Landfill has low impacts on most
HFO1234ze, with shares of 82%, 75% and 89%, of the categories.
although this is only used in a small amount in the XPS The energy recovery from thermal treatment of the
product with 5% of the raw material input. The high used XPS-boards generates a relevant amount of
contribution of HFO is in parts unexpected and strongly energy.
7. Requisite evidence
7.1 VOC Emissions AgBB overview of results (28 days [µg/m³])
Name Value Unit
JACKODUR Plus can be used indoor however it is TVOC (C6 - C16) 0 μg/m3
generally not exposed to the indoor air but covered by Sum SVOC (C16 - C22) 0 μg/m3
a finishing element or system. R (dimensionless) 0 -
The emissions of JACKODUR Plus have been tested VOC without NIK 0 μg/m3
by TÜV Rheinland, Germany in March 2015 following Carcinogenic Substances 0 μg/m3
EN ISO 16000.
AgBB overview of results (3 days [µg/m³])
The emission testing met the requirements of the Name Value Unit
Committee for Health-related Evaluation of Building TVOC (C6 - C16) 21 μg/m3
Products/German Institute for Structural Engineering Sum SVOC (C16 - C22) 0 μg/m3
(AgBB) method. The tested products all complied with
R (dimensionless) 0.022 -
the requirements of AgBB (May 2010) for the use in
VOC without NIK 7 μg/m3
the indoor environment. The tested products also all
Carcinogenic Substances 0 μg/m3
achieved the A+ rating of the French Volatile Organic
Compound (VOC) labelling scheme (TÜV report).
7.2 Leaching performance
Leaching behaviour is not regulated for extruded
polystyrene foam products.
8. References
EN 15804 Environmental Declarations – Basic principles and
EN 15804:2012-04+A1 2013, Sustainability of procedures
construction works – Environmental product
declarations – Core rules for the product category of AgBB
construction products Indoor air quality requirements in buildings: Health
evaluation of volatile organic compounds (VVOC, VOC
IBU 2019 and SVOC) emissions from construction products,
Institut Bauen und Umwelt e.V.: General Programme German Committee for Health-Related Evaluation of
Instructions for the Preparation of EPDs at the Institut Building Products, 2010
Bauen und Umwelt e.V., version 1.8, Berlin: Institut
Bauen und Umwelt e.V., 2019, http://www.ibu-epd.com AVV
Ordinance concerning the European Waste Directory
ISO 14025 (Waste Directory Ordinance - AVV): Waste Directory
DIN EN ISO 14025:2011-10, Ordinance dated 10th December 2011 (Federal Legal
Environmentaldesignations and declarations – Type III Gazette I p. 3379), which has been modified by Article
7 Environmental Product Declaration Jackon Insulation GmbH – XPS Foam Insulation Jackodur plus
5 Paragraph 22 of the law dated 24th February 2012 DIN EN ISO 16000-1:2006-06, Indoor air - Part 1:
(Federal Legal Gazette. I p. 212). General aspects of sampling strategy (ISO 16000-
1:2004); German version EN ISO 16000-1:2006
DIBt
German Institute for Construction Technology, Berlin GaBi ts
www.dibt.de GaBi ts Software and Documentation: Database for
integrated balancing. LBP, University of Stuttgart and
Ecoinvent database thinkstep AG, Documentation of GaBi ts data sets,
Ecoinvent data base, Version v2-2, http://www.gabi-
www.ecoinvent.org, 2010 software.com/deutsch/datenbanken/gabi-datenbanken,
2020
EN 12088
2013-06: Thermal insulation products for building IPCC 2013
applications – Determination of long-term water Climate Change 2013: The Physical Science Basis.
absorption by diffusion Contribution of Working Group I to the Fifth
Assessment Report of the Intergovernmental Panel on
EN 12091 Climate Change (IPCC), Cambidge University Press,
2013-06: Thermal insulation products for building Cambridge, United Kingdom and New York, NY, USA
applications – Determination of freeze-thaw resistance
ISO 9001
EN 826 ISO 9001: 2015, Quality management systems -
2013-05: Thermal insulation products for building Requirements
applications – Determination of compression behaviour
ISO 15686
EN 13501-1 ISO 15686-2:2012-05, Buildings and constructed
EN 13501-1 + A1: 2018, Fire classification of assets - Service life planning - Part 2: Service life
construction products and building elements - Part 1: prediction procedures
Classification using data from reaction to fire tests
ISO 50001
EN 12667 Energy management systems – Requirements with
2001-05: Thermal performance of buildings materials guidance for use
and products – Determination of thermal resistance by
means of guarded hot plate and heat flow meter ISO 14001
methods - Products of high and medium thermal ISO 14001: 2015, Environmental management
resistance systems - Requirements with guidance for use
EN 13164 PCR, Part A
EN 13164: 2012 + A1: 201, Thermal insulation PCR 2018 - Part A, Calculation rules for the Life Cycle
products for buildings – Factory-made extruded Assessment and Requirements on the Background
polystyrene foam (XPS) products – Specification Report, Version 1.7, Institut Bauen und Umwelt e.V.,
2018, www.bau-umwelt.com
EN 1604
EN 1604:2013-05: Thermal insulating products for PCR, Part B
building applications – Determination of dimensional Product category rules for construction products Part
stability under specified temperature and humidity B: Requirements of the EPD for foam plastic insulation
conditions materials, version 1.7, 2019, www.bau-umwelt.de
EN 1605 REACH
EN 1605:2013-05: Thermal insulating products for Regulation (EC) No 1907/2006 concerning the
building applications – Determination of deformation Registration, Evaluation, Authorisation and Restriction
under specified compressive load and temperature of Chemicals
conditions
TÜV Rheinland, Germany
EN 1606 Global provider of technical, safety, and certification
2013-05: Thermal insulating products for building services; headquarter Cologne, Germany
applications – Determination of compressive creep www.tuv.com
EN 1607 TÜV report
2013-05 Thermal insulating products for building TÜVRheinland, Test report No.: 21230643 001, VOC
applications – Determination of tensile strength measuring results for Jackodur Plus, TÜV Rheinland
perpendicular to face LGA Products GmbH, 2015
EN 12086 Ullmanns
2013-06: Thermal insulation products for building John Wilay & Sons, Inc., ULLMANN'S Encyclopedia of
applications – Determination of water vapour trans- Industrial Chemistry, Hoboken / USA, 2014
mission properties
EN ISO 16000
8 Environmental Product Declaration Jackon Insulation GmbH – XPS Foam Insulation Jackodur plus
Publisher
Institut Bauen und Umwelt e.V. Tel +49 (0)30 3087748- 0
Panoramastr. 1 Fax +49 (0)30 3087748- 29
10178 Berlin Mail info@ibu-epd.com
Germany Web www.ibu-epd.com
Programme holder
Institut Bauen und Umwelt e.V. Tel +49 (0)30 - 3087748- 0
Panoramastr 1 Fax +49 (0)30 – 3087748 - 29
10178 Berlin Mail info@ibu-epd.com
Germany Web www.ibu-epd.com
Author of the Life Cycle
Assessment Tel +49 711 341817-0
Sphera Solutions GmbH Fax +49 711 341817-25
Hauptstraße 111- 113 Mail info@sphera.com
70771 Leinfelden-Echterdingen Web http://www.sphera.com
Germany
Owner of the Declaration
JACKON Insulation GmbH Tel +49 5204 9955-0
Carl-Benz-Straße 8 Fax +49 5204 9955-400
33803 Steinhagen Mail info@jackon.com
Germany Web www.jackon-insulation.com
