ENVIRONMENTAL PRODUCT DECLARATION
as per ISO 14025 and EN 15804+A2
Owner of the Declaration James Hardie Europe GmbH
Publisher Institut Bauen und Umwelt e.V. (IBU)
Programme holder Institut Bauen und Umwelt e.V. (IBU)
Declaration number EPD-JAM-20240184-IBA1-EN
Issue date 15.08.2024
Valid to 14.08.2029
Aestuver® Tx Fire protection board
James Hardie Europe GmbH
www.ibu-epd.com | https://epd-online.com
1. General Information
James Hardie Europe GmbH Aestuver® Tx Fire protection board
Programme holder Owner of the declaration
IBU – Institut Bauen und Umwelt e.V. James Hardie Europe GmbH
Hegelplatz 1 Bennigsen­Platz 1
10117 Berlin 40474 Düsseldorf
Germany Germany
Declaration number Declared product / declared unit
EPD­JAM­20240184­IBA1­EN 1 m² Aestuver® Tx Fire protection board
This declaration is based on the product category rules: Scope:
Fibre cement / Fibre concrete, 01.08.2021 This document refers to the manufacture of Aestuver® Tx Fire protection
(PCR checked and approved by the SVR) boards by James Hardie Europe GmbH. This product is produced in the
manufacturing plant in Calbe/Germany in which the production data for
2022 was recorded. The Life Cycle Assessment therefore fully represents
Issue date the Aestuver® Tx Fire protection boards produced in Calbe by James
15.08.2024 Hardie Europe GmbH.
The owner of the declaration shall be liable for the underlying information
and evidence; the IBU shall not be liable with respect to manufacturer
Valid to information, life cycle assessment data and evidences.
14.08.2029 The EPD was created according to the specifications of EN 15804+A2. In
the following, the standard will be simplified as EN 15804.
Verification
The standard EN 15804 serves as the core PCR
Independent verification of the declaration and data according to ISO
14025:2011
internally X externally
Dipl.­Ing. Hans Peters
(Chairman of Institut Bauen und Umwelt e.V.)
Florian Pronold Dr.­Ing. Nikolay Minkov,
(Managing Director Institut Bauen und Umwelt e.V.) (Independent verifier)
1 Environmental Product Declaration ­ James Hardie Europe GmbH ­ Aestuver® Tx Fire protection board
2. Product
2.1 Product description/Product definition 2.5 Base materials/Ancillary materials
Aestuver® Tx Fire protection boards are cement­bound, Base materials weight as percentage
fibreglass­reinforced lightweight concrete boards manufactured
Name Value Unit
in thicknesses of 20 to 60 mm. The boards have sandwich
M­
structure, i.e. they comprise surface layer and core material cement: binder 50­80
%
components whose mass ratio varies with thickness. Both
cover layers, which comprise the top and bottom of the core of M­
fly ash: binder/ filler 0­10
the panel, are around 3 mm thick. The material of the top layer %
and the core are made from the same raw materials, but in M­
CSH: filler 0­15
different compositions.. %
Placing on the market / Application rules M­
The placing on the market of the product in the EU / EFTA (with Perlite: leightweight aggregates 5­35 %
the exception of Switzerland) is governed by Regulation (EU)
M­
No 305/2011 / CPR. The product requires a declaration of Alkali­resistant glassfibre: reinforcement 0,5­5
%
performance taking into account the / European Technical
Plasticisers, stabilising agents, air­entraining aprox. M­
Assessment No. ETA-17/0170 and the CE marking. The
agents: Auxiliaries/ Additives 1 %
declaration of performance has been prepared: Aestuver® Tx
Fire protection board FC­0010. Additional additives such as flame retardants, softeners or
For use, the respective national regulations apply. biocides are not used in the production of Aestuver® Tx Fire
protection boards.
2.2 Application
Aestuver® Tx Fire protection boards for tunnel use are used in This product/article/at least one partial article contains
precautionary structural fire protection as concreted or substances listed in the candidate list (date: 18.12.2006)
subsequently fastened cladding for the protection of exceeding 0.1 percentage by mass: no
construction concrete in tunnels.
Aestuver® Tx Fire protection boards are also used as building This product/article/at least one partial article contains other
and fire protection boards for partition walls, as fire protection CMR substances in categories 1A or 1B which are not on the
paneling of components and elements, as well as interior and candidate list, exceeding 0.1 percentage by mass: no
exterior cladding, as plaster base boards for facades and
ceilings, and as fire protection products for technical building Biocide products were added to this construction product or it
equipment and as components of fire resistant components. has been treated with biocide products (this then concerns a
treated product as defined by the (EU) Ordinance on Biocide
2.3 Technical Data
Products No. 528/2012): no
Aestuver® Tx Fire protection board (depends on thickness).
2.6 Manufacture
Constructional data
The production of the Aestuver® Tx Fire protectionn boards
Name Value Unit
takes place in a completely automated production process on a
Thermal conductivity DIN EN 12667 0.15 ­ W/(mK) production line in layers "fresh in fresh" in steel moulds. In a
0.25 first step, the lower cover layer is sprayed into the mould
Water vapour diffusion resistance factor acc. together with glass fibre segments cut from a continuous
10 ­ 12 ­
to DIN V 4108­4, EN ISO 12572 strand. Immediately afterwards, the core layer is applied onto
Swelling (air­dry to water­saturated) 1 mm/m the fresh lower cover layer from a distributor station. In a final
Gross density DIN EN 12467 800 kg/m3 step, the upper, covering cover layer is sprayed onto a carrier
film, deposited on the core layer and rolled on.
Compressive strength DIN EN 789 3.5 N/mm2
The finished rough strand is then cut according to the mould
Tensile strength DIN EN 319 0.3 N/mm2 size, the filled moulds are stacked separately and linger for
Flexural strength DIN EN 12467 1.5 N/mm2 several hours in a setting channel. In the demoulding station,
the hardened boards are removed from the moulds, placed on
Modulus of elasticity DIN EN 12467 2000 N/mm2
stacking grids and dried in the drier to the delivery moisture.
Moisture content at 23 °C, 80% humidity at 5 M.­% After the drying time, the boardss are trimmed by the edges,
23 °C, 80% humidity at 20°C, 65% calibrated in thickness, palletized and packaged. The boards
Coefficient of thermal expansion 0.01 10­6K­1 remain in stock until a maturation period has elapsed.
Chemical resistance DIN EN 12467/, X, Y, Z1,
category of use acc. ETAG 018­1 Z2 ­ The manufacturing plant has been certified a quality
management system according to DIN EN ISO 9001: 2015 by
Ageing resistance DIN EN 12467/, category X, Y, Z1,
­ TÜV Nord since 2010 and operates a system of factory
of use acc. ETAG 018­1 Z2
production control oriented to the requirements of the European
Permanent temperature resistance 105 °C
Technical Assessment and Product Safety Regulations. In
Performance data of the product in accordance with the addition to the incoming goods inspection and the permanent
declaration of performance with respect to its essential production monitoring, this includes the final inspection of the
characteristics according ETA-17/0170. finished products.
2.4 Delivery status 2.7 Environment and health during manufacturing
The boards are manufactured in a range of thicknesses from 20 During production of Aestuver® Tx Fire protection boards,
mm to 60 mm. The boards can be up to 3000 mm in length and exclusively low­chromate (< 2ppm) cement is used in
up to 1250 mm wide. accordance with RL 2003/53/EG and the REACH Directive
2 Environmental Product Declaration ­ James Hardie Europe GmbH ­ Aestuver® Tx Fire protection board
(EC), Annex XVII, No. 1907/2006. Excess process water or
cleaning water is mechanically filtered in the process water 2.13 Extraordinary effects
circuit in order to separate cleaning residue. The cleaned water Fire
is added to the manufacturing process as service water. In accordance with the 96/603/EG and 2000/605/EG rulings by
Noise: the European Commission, uncoated Aestuver® Tx Fire
Sound protection analyses have established that all values protection boards are classified as Class A1, non­combustible
communicated inside and outside the production facility are far building materials according to DIN EN 13501-1. In addition,
below the requisite technical standards. they are also Class A1 non­combustible building materials
Waste: according to DIN 4102.
All types of waste such as scrap metal, waste oil, foils and Water
plastic chips (packaging), wood (pallets) and paper are Aestuver® Tx Fire protection boards display neutral reaction
separated, stored and directed back into the recycling system. when exposed to water (e.g. flooding). No substances are
washed out which could be hazardous to water.
2.8 Product processing/Installation
Aestuver® Tx Fire protection board cuttings are achieved using Mechanical destruction
conventional rail­guided hand­held circular saws with suction, Not relevant.
preferably as plunge­cut sawing. For precisely fitting and sharp­
edged cuts, the use of carbide­tipped saw blades with 2.14 Re-use phase
alternating teeth is recommended. The dust content is reduced Cement­bound lightweight concrete boards can be easily
by the use of saw blades with a small number of teeth and at deconstructed. They do not need to be treated as special waste
low speeds. The attachment is done by means of drywall when demolished / deconstructed. With regard to an efficient
screws or by means of commercial staples. recycling process, care should be exercised in ensuring
dismantling whereby waste is sorted into as many different
2.9 Packaging categories as possible.
Aestuver® Tx Fire protection boards are packed lying on Reuse and further use
wooden pallets and supplied with cardboard edge protection Cement­bound lightweight concrete boards usually outlast the
and covered with foil. These packaging materials are separated service life of the buildings in which they are used. After
and returned to the recycling circuit. The wooden pallets can be deconstructing such buildings, the materials can therefore be
returned to the respective dealers. prepared, classified, assessed (environmental compatibility,
building material characteristic values, consistency) and
2.10 Condition of use reused. The waste incurred by these boards and any
Due to the stable crystalline calcium­silicate hydrate phase components manufactured from them can be recovered in
binding and achieved after curing solid structure emissions are building material recycling plants before being used as an
normal for the intended use of the products described use, aggregate for various applications. Unmixed residual materials
extremely low and are considered to be harmless to health. No can be taken by the manufacturers and re­used or recycled.
risks are associated with water, air and soil if the products are This material can be used as aggregates in production. Building
used as intended. The natural ionizing radiation of Aestuver® rubble and production rejects should be prepared mixed to
Tx Fire protection boards is extremely low and harmless to ensure the consistent features of lightweight concrete products
health hazards. made from recycled material. The recycled material should
comply with the natural requirements of the material standards
2.11 Environment and health during use
for the raw material to be replaced. Furthermore, recycled
The Institut für Baubiologie in Rosenheim has tested Aestuver® material made from lightweight concrete can also be used for
Tx Fire protection boards and their manufacturing process with building roads and paths in construction class V.
regard to healthy living and environmental protection (xxx).
2.15 Disposal
2.12 Reference service life
If in exceptional cases, materials can not be directed to a
A service life of at least 25 years has been confirmed by test building material recycling plant, the Aestuver® Tx Fire
scenarios for Aestuver® Tx Fire protection boards. The practical protection boards can be disposed of at any building rubble
service life can however be much longer. However, the landfill in accordance with the /waste key number 170101/
indications given on the working life can not be interpreted as a (concrete).
guarantee given by the manufacturer, but are to be regarded
only as a means of selecting the right products in relation to the 2.16 Further information
expected economically reasonable working life of the works. Further information on the products is available in the
The prerequisite for a long service life is that the necessary Download area on www.fermacell.com. Safety data sheets can
conditions for packaging, transport, storage, installation, use, be requested by calling 0800 5235665.
maintenance and repair and maintenance have been met
(please refer to www.aestuver.com).
3. LCA: Calculation rules
the Calbe plant.
3.1 Declared Unit
Name Value Unit
Declared unit and mass reference Declared unit 1 m²
This declaration refers to the manufacture of 1m² Aestuver® Tx Grammage 28.6 kg/m2
Fire protection board by James Hardie Europe GmbH. The
Layer thickness 0,035 m
boards are manufactured in varying thicknesses. The average
grammage of fire­resistant boards produced is 28,6 kg/m² Gross density 818 kg/m3
(complies with a board of approx. 35mm thickness). The conversion factor to 1 kg 0.035 ­
average was based on the annual production volume 2022 at
3 Environmental Product Declaration ­ James Hardie Europe GmbH ­ Aestuver® Tx Fire protection board
3.2 System boundary 3.4 Cut-off criteria
Type of the EPD: cradle to gate with Options All data from the production data collection, i.e. all raw
materials used according to the recipe, their transport to the
The EPD considers module A1­A3, A4, A5, C1­C4 and D plant, the thermal and electrical energy used, packaging
materials, all direct production waste and all available emission
Module A1 includes provision of all raw materials and pre­ measurements were taken into account in the balance. In this
products (for example cement) and energy supply, as well as way, material and energy flows with a share of less than one
waste processing up to the end­of waste state or disposal of percent were also taken into account.
final residues during the product stage. Machinery, equipment and infrastructure required for production
were neglected and thus not considered.
Module A2 considers the transport of these raw materials to The sum of the excluded material flows does not exceed 5% of
James Hardie's production site located in Germany via truck. mass, energy or environmental relevance.
Module A3 considers the manufacturing of the product in 3.5 Background data
James Hardie's production site including the provision of The background data are taken from the Sphera LCA FE
electricity and thermal energy from natural gas. The production (former GaBi databases).
of packaging materials is also included.Manufacturing losses
3.6 Data quality
are close to zero and thus not considered in the LCA.
All primary data are collected for the year 2022. All secondary
Module A4 considers 100 km truck transport to site. The data come from the Sphera LCA FE (GaBi) databases and are
transport distance can be modified project specific if required by representative of the years 2018­2023. As the study intended to
linear scaling. compare the product systems for the reference year, temporal
representativeness is good.
Module A5 considers the treatment and disposal of packaging The overall technological and geographical representativeness
material. Credits for potential avoided burdens due to energy is also considered to be good.
substitution of electricity and thermal energy generation are
3.7 Period under review
declared in module D.
Primary production data were collected in James Hardie's
production site in Calbe, based on the annual production
Module C1 considers the dismantling of the product at EoL with
volume 2022.
an Excavator, 100 kW.
3.8 Geographic Representativeness
Module C2 accounts for a 50 km transport by truck.
Land or region, in which the declared product system is
manufactured, used or handled at the end of the product´s
Two scenarios are considered in the End­of­life; recycling (1)
lifespan: Germany
and landfilling (2).
Module C3 (Scenario 1) calculates the recycling processing 3.9 Allocation
efforts, in which the entire product is processed and a material The production process does not deliver any co­products. The
credit for roadworks (gravel) is applied in module D. For C3/1 data were collected product specific.
the results are '0'. Fly ash, like all other power plant by­products, is allocated by
market value.
Module C4/1 (Scenario 2) considers landfilling of the product.
For C4 the results are '0'. All applied incineration processes (module A5) are displayed
via a partial stream consideration for the combustion process,
Module D includes potential benefits for the thermal and according to the specific composition of the incinerated
electrical energy generated in module A5 due to packaging material. For the waste incineration plant an R1­value of 0.6 is
treatment and also the material credit due to the product assumed.
processing in module C3. Avoided burdens have been Environmental burden of the incineration of packaging are
calculated by the inversion of electricity grid mix and thermal assigned to the system (A5); resulting credits for thermal and
energy from natural gas. The material credit is calculated by electrical energy are declared in module D.
using a generic data set for gravel. The credits for thermal and electrical energy are calculated via
inversion of the life cycle inventory of average data.
Module D/1 accounts for the avoided burdens for electricity grid
mix and thermal energy from natural gas due to packaging 3.10 Comparability
incineration resulting from A5 only. Basically, a comparison or an evaluation of EPD data is only
possible if all the data sets to be compared were created
3.3 Estimates and assumptions
according to EN 15804 and the building context, respectively
For electricity production the Residual Grid mix for Germany is the product­specific characteristics of performance, are taken
accounted for within the LCA. into account. The used background database is Sphera LCA
FE (former GaBi database), CUP2023.1
4. LCA: Scenarios and additional technical information
Information on describing the biogenic carbon content at
Characteristic product properties of biogenic carbon
factory gate
The product itself does not contain any biogenic carbon. Only
the packaging (wooden pallets, paper) does contain it.
Note: 1 kg of biogenic carbon is equivalent to 44/12 kg of CO2
4 Environmental Product Declaration ­ James Hardie Europe GmbH ­ Aestuver® Tx Fire protection board
Name ValueUnit due to the energy generation after incineration are assigned to
module D.
kg
Biogenic carbon content in product ­
C Name Value Unit
Biogenic carbon content in accompanying kg wooden pallet 0.48 kg
0.2
packaging C paper 0.003 kg
plastic foil 0.002 kg
End of life (C1-C4)
Transport to the building site (A4)
Name Value Unit
This module considers 100 km truck transport to site (diesel
Collected as mixed construction waste 28.6 kg
driven). The transport distance can be modified project specific
if required by linear scaling. Recycling 28.6 kg
Name Value Unit Landfilling 28.6 kg
Litres of fuel 0.08 l/100km Module D considers the benefits of packaging treatment (from
Transport distance 100 km Module A5) and material credit after waste processing (from
Module C3)
Capacity utilisation (including empty runs) 61 %
Installation into the building (A5) Module D/1 considers the benefits of packaging treatment (from
Module A5) only
The following packaging materials come with the declared
product and are incinerated after installation. Potential benefits
5 Environmental Product Declaration ­ James Hardie Europe GmbH ­ Aestuver® Tx Fire protection board
5. LCA: Results
The following table shows the results for 1m² Aestuver® Tx Fire protection board. The recycling scenario (EoL1) shows the
corresponding results in C3, for C3/1 the results are '0'.
The landfill scenario (EoL2) shows the results in C4/1, for C4 the results are '0'.
Moreover, only packaging incineration ends up in potential benefits in D/1. Module D includes besides those benefits also the material
credit due to recycling.
DESCRIPTION OF THE SYSTEM BOUNDARY (X = INCLUDED IN LCA; MND = MODULE OR INDICATOR NOT DECLARED; MNR
= MODULE NOT RELEVANT)
Benefits and
Construction loads beyond
Product stage Use stage End of life stage
process stage the system
boundaries
la ire ta m w a Ry lp p u s tro p s n a rT g n iru tc a fu n a M e h t m o rf tro p s n a rTe tis e h t o t e ta g y lb m e s s A e s U e c n a n e tn ia M ria p e R tn e m e c a lp e R tn e m h s ib ru fe R y g re n e la n o ita re p Oe s u re ta w la n o ita re p Oe s u n o itc u rts n o c ­e Dn o itilo m e d tro p s n a rT g n is s e c o rp e ts a W la s o p s iD ­e s u e R­y re v o c e R­g n ilc y c e Rla itn e to p
A1 A2 A3 A4 A5 B1 B2 B3 B4 B5 B6 B7 C1 C2 C3 C4 D
X X X X X MND MND MNR MNR MNR MND MND X X X X X
RESULTS OF THE LCA - ENVIRONMENTAL IMPACT according to EN 15804+A2: 1 m² Aestuver® Tx Fire protection board
Parameter Unit A1-A3 A4 A5 C1 C2 C3 C3/1 C4 C4/1 D D/1
GWP­total kg CO 2 eq 3.41E+01 2.46E­01 8.92E­01 1.75E­02 1.23E­01 7.45E­02 0 0 4.33E­01 ­3.55E­01 ­3.01E­01
GWP­fossil kg CO 2 eq 3.47E+01 2.16E­01 2.03E­02 1.54E­02 1.08E­01 7.42E­02 0 0 4.3E­01 ­3.54E­01 ­2.98E­01
GWP­
biogenic kg CO 2 eq ­6.38E­01 2.82E­02 8.72E­01 2.03E­03 1.41E­02 1.13E­05 0 0 1.75E­03 ­1.34E­03 ­2.69E­03
GWP­luluc kg CO 2 eq 1.07E­02 1.47E­03 2.23E­06 1.02E­04 7.33E­04 3.58E­04 0 0 1.34E­03 ­2.65E­04 ­2.72E­05
kg CFC11
ODP 1.85E­11 4.29E­14 1.33E­13 3E­15 2.14E­14 2.23E­13 0 0 1.09E­12 ­3.98E­12 ­3.62E­12
eq
AP mol H+ eq 3.97E­02 1.82E­04 1.61E­04 8.56E­05 9.09E­05 3.71E­04 0 0 3.05E­03 ­5.83E­04 ­2.99E­04
EP­
kg P eq 1.01E­05 5.71E­07 3.21E­08 3.99E­08 2.86E­07 1.93E­07 0 0 8.66E­07 ­1.08E­06 ­8.02E­07
freshwater
EP­marine kg N eq 9.76E­03 4.77E­05 4.51E­05 4.07E­05 2.38E­05 1.73E­04 0 0 7.88E­04 ­2.11E­04 ­1.11E­04
EP­terrestrial mol N eq 1.08E­01 6.3E­04 7.73E­04 4.5E­04 3.15E­04 1.91E­03 0 0 8.67E­03 ­2.28E­03 ­1.18E­03
kg NMVOC
POCP 2.77E­02 1.47E­04 1.18E­04 1.14E­04 7.35E­05 4.67E­04 0 0 2.38E­03 ­5.57E­04 ­2.85E­04
eq
ADPE kg Sb eq 7.11E­07 1.74E­08 9.92E­10 1.21E­09 8.68E­09 7.93E­08 0 0 1.98E­08 ­3.16E­08 ­2.58E­08
ADPF MJ 2.95E+02 3.32E+00 2.04E­01 2.32E­01 1.66E+00 1.43E+00 0 0 5.72E+00 ­5.51E+00 ­4.65E+00
m3 world eq
WDP 3.84E­01 1.28E­03 9.14E­02 8.91E­05 6.38E­04 1.29E­02 0 0 4.72E­02 ­9.8E­03 ­3.91E­03
deprived
GWP = Global warming potential; ODP = Depletion potential of the stratospheric ozone layer; AP = Acidification potential of land and water; EP =
Eutrophication potential; POCP = Formation potential of tropospheric ozone photochemical oxidants; ADPE = Abiotic depletion potential for non­fossil
resources; ADPF = Abiotic depletion potential for fossil resources; WDP = Water (user) deprivation potential)
RESULTS OF THE LCA - INDICATORS TO DESCRIBE RESOURCE USE according to EN 15804+A2: 1 m² Aestuver® Tx Fire
protection board
Parameter Unit A1-A3 A4 A5 C1 C2 C3 C3/1 C4 C4/1 D D/1
PERE MJ 1.19E+01 2.15E­01 8.84E+00 1.5E­02 1.07E­01 1.57E­01 0 0 9.33E­01 ­2.04E+00 ­1.76E+00
PERM MJ 8.77E+00 0 ­8.77E+00 0 0 0 0 0 0 0 0
PERT MJ 2.06E+01 2.15E­01 6.49E­02 1.5E­02 1.07E­01 1.57E­01 0 0 9.33E­01 ­2.04E+00 ­1.76E+00
PENRE MJ 2.94E+02 3.33E+00 5.53E­01 2.32E­01 1.66E+00 1.43E+00 0 0 5.73E+00 ­5.51E+00 ­4.65E+00
PENRM MJ 3.49E­01 0 ­3.49E­01 0 0 0 0 0 0 0 0
PENRT MJ 2.95E+02 3.33E+00 2.05E­01 2.32E­01 1.66E+00 1.43E+00 0 0 5.73E+00 ­5.51E+00 ­4.65E+00
SM kg 2.92E+00 0 0 0 0 0 0 0 0 0 0
RSF MJ 0 0 0 0 0 0 0 0 0 0 0
NRSF MJ 0 0 0 0 0 0 0 0 0 0 0
FW m3 3.26E­02 1.96E­04 2.15E­03 1.37E­05 9.79E­05 3.77E­04 0 0 1.45E­03 ­8.82E­04 ­6.26E­04
PERE = Use of renewable primary energy excluding renewable primary energy resources used as raw materials; PERM = Use of renewable primary
energy resources used as raw materials; PERT = Total use of renewable primary energy resources; PENRE = Use of non­renewable primary energy
excluding non­renewable primary energy resources used as raw materials; PENRM = Use of non­renewable primary energy resources used as raw
materials; PENRT = Total use of non­renewable primary energy resources; SM = Use of secondary material; RSF = Use of renewable secondary fuels;
NRSF = Use of non­renewable secondary fuels; FW = Use of net fresh water
RESULTS OF THE LCA – WASTE CATEGORIES AND OUTPUT FLOWS according to EN 15804+A2:
1 m² Aestuver® Tx Fire protection board
Parameter Unit A1-A3 A4 A5 C1 C2 C3 C3/1 C4 C4/1 D D/1
HWD kg 1.58E­08 8.91E­12 2.28E­12 6.23E­13 4.45E­12 0 0 0 1.25E­10 ­2.68E­10 ­2.89E­10
6 Environmental Product Declaration ­ James Hardie Europe GmbH ­ Aestuver® Tx Fire protection board
NHWD kg 3.83E+00 4.85E­04 6.69E­03 3.39E­05 2.42E­04 4E­04 0 0 2.87E+01 ­1.16E+00 ­2.49E­03
RWD kg 4.32E­03 3.48E­06 6.75E­06 2.43E­07 1.74E­06 1.17E­05 0 0 6.52E­05 ­2.41E­04 ­1.82E­04
CRU kg 0 0 0 0 0 0 0 0 0 0 0
MFR kg 0 0 0 0 0 2.86E+01 0 0 0 0 0
MER kg 0 0 0 0 0 0 0 0 0 0 0
EEE MJ 0 0 1.09E+00 0 0 0 0 0 0 0 0
EET MJ 0 0 2.55E+00 0 0 0 0 0 0 0 0
HWD = Hazardous waste disposed; NHWD = Non­hazardous waste disposed; RWD = Radioactive waste disposed; CRU = Components for re­use;
MFR = Materials for recycling; MER = Materials for energy recovery; EEE = Exported electrical energy; EET = Exported thermal energy
RESULTS OF THE LCA – additional impact categories according to EN 15804+A2-optional:
1 m² Aestuver® Tx Fire protection board
Parameter Unit A1-A3 A4 A5 C1 C2 C3 C3/1 C4 C4/1 D D/1
Disease
PM 6.62E­07 1.32E­09 8.52E­10 9.79E­10 6.6E­10 7.19E­09 0 0 3.75E­08 ­1.88E­08 ­2.18E­09
incidence
IR kBq U235 eq 3.72E­01 3.58E­04 7.17E­04 2.5E­05 1.79E­04 1.23E­03 0 0 7.53E­03 ­2.9E­02 ­1.93E­02
ETP­fw CTUe 1E+02 2.47E+00 8.2E­02 1.73E­01 1.24E+00 1.02E+00 0 0 3.12E+00 ­1.26E+00 ­7.85E­01
HTP­c CTUh 2.3E­09 4.93E­11 6.06E­12 3.45E­12 2.47E­11 2.24E­11 0 0 4.81E­10 ­9.33E­11 ­5.63E­11
HTP­nc CTUh 1.43E­07 2.43E­09 1.98E­10 2.01E­10 1.22E­09 1.12E­09 0 0 5.29E­08 ­5.37E­09 ­1.76E­09
SQP SQP 1.39E+02 1.18E+00 7.02E­02 8.25E­02 5.9E­01 3.6E­01 0 0 1.39E+00 ­1.51E+00 ­1.22E+00
PM = Potential incidence of disease due to PM emissions; IR = Potential Human exposure efficiency relative to U235; ETP­fw = Potential comparative
Toxic Unit for ecosystems; HTP­c = Potential comparative Toxic Unit for humans (cancerogenic); HTP­nc = Potential comparative Toxic Unit for humans
(not cancerogenic); SQP = Potential soil quality index
Disclaimer 1 – for the indicator “Potential Human exposure efficiency relative to U235”. This impact category deals mainly with the
eventual impact of low­dose ionizing radiation on human health of the nuclear fuel cycle. It does not consider effects due to possible
nuclear accidents, occupational exposure or radioactive waste disposal in underground facilities. Potential ionizing radiation from the
soil, radon and from some construction materials is also not measured by this indicator.
Disclaimer 2 – for the indicators “abiotic depletion potential for non­fossil resources”, “abiotic depletion potential for fossil resources”,
“water (user) deprivation potential, deprivation­weighted water consumption”, “potential comparative toxic unit for ecosystems”,
“potential comparative toxic unit for humans – cancerogenic”, “Potential comparative toxic unit for humans ­ not cancerogenic”,
“potential soil quality index”. The results of this environmental impact indicator shall be used with care as the uncertainties on these
results are high as there is limited experience with the indicator.
6. LCA: Interpretation
Life Cycle: The main drivers of the manufacturing phase in most impact
The manufacturing phase dominates the product system. In categories are the raw materials cement, blown perlite and
addition, the packaging treatment in module A5 has relevant glass fibres. Electrical and thermal energy consumption in the
environmental impacts where the credits accounted in module product manufacture is reflected with relevant contributions in
D cover the inversion of electricity grid mix and thermal energy most of the indicators. The resource use minerals and metals
from natural gas due to packaging treatment (A5). The impacts contribution seem maximum from aerated concrete. The
from the C4/2 scenario are comparatively higher than the biogenic carbon content in the wooden pallets is reflected by
results of the C3/1 scenario. the higher negative contributions in GWP biogenic.
Product stage:
7. Requisite evidence
The Institut für Baubiologie in Rosenheim has tested Aestuver® Name Value Unit
Tx Fire protection boards and their manufacturing process with Arsenic (As) 0,001 mg/l
regard to healthy living and environmental protection (xxx).
Cadmium (Cd) 0,0003 mg/l
Thalium (Ti) 0,0002 mg/l
7.1 Radioactivity
Assessment performed on the basis of: Chromium (Cr) 0,001 mg/l
­ EU Commission "Radiation Protection 112" document Nickel (Ni) 0,001 mg/l
(MPA NRW, Test report No. 321000741 ) Copper (Cu) 0,005 mg/l
Determination of Radioactivity Mercury (Hg) 0,0002 mg/l
Name Value Unit Zinc (Zn) 0,01 mg/l
Radium­226 120 ± 5 Bq/kg Lead (Pb) 0,001 mg/l
Radium­228 120 ± 4 Bq/kg 7.3 VOC emissions
Thorium­228 120 ± 10 Bq/kg Test procedure in line with the AgBB
Potassium­40 140 ± 20 Bq/kg (MPA Eberswalde, Report No. 31/24/5372/01)
AgBB overview of results (28 days [µg/m³])
7.2 Leaching
Eluate analysis to DIN 38414, Part 4
(Eurofin Umwelt Ost, Expert Report No. AR­24­KS­001439­01)
Determination of the eluate
7 Environmental Product Declaration ­ James Hardie Europe GmbH ­ Aestuver® Tx Fire protection board
Name Value Unit Name Value Unit
TVOC (C6 ­ C16) 5 μg/m3 TVOC (C6 ­ C16) 210 μg/m3
Sum SVOC (C16 ­ C22) 5 μg/m3 Sum SVOC (C16 ­ C22) 5 μg/m3
R (dimensionless) 0.004 ­ R (dimensionless) 0.18 ­
VOC without NIK < 5 μg/m3 VOC without NIK 126 μg/m3
Carcinogenic Substances < 1 μg/m3 Carcinogenic Substances < 1 μg/m3
AgBB overview of results (3 days [µg/m³])
8. References
Standards
REACH-Verordnung (EG)
EN 15804 REGULATION (EC) No 1907/2006 OF THE EUROPEAN
EN 15804:2012+A2:2019+AC:2021, Sustainability of PARLIAMENT AND OF THE COUNCIL of 18 December 2006
construction works — Environmental Product Declarations — concerning the Registration, Evaluation, Authorisation and
Core rules for the product category of construction products. Restriction of Chemicals (REACH), establishing a European
Chemicals Agency, amending Directive 1999/45/EC and
repealing Council Regulation (EEC) No 793/93 and
ISO 14025 Commission Regulation (EC) No 1488/94 as well as Council
EN ISO 14025:2011, Environmental labels and declarations — Directive 76/769/EEC and Commission Directives 91/155/EEC,
Type III environmental declarations — Principles and 93/67/EEC, 93/105/EC and 2000/21/EC.
procedures.
(EU) Nr. 305/2011 (CPR)
Further References REGULATION (EU) No 305/2011 OF THE EUROPEAN
PARLIAMENT AND OF THE COUNCIL.
Sphera LCA FE (former GaBi ts)
Sphera LCA for Experts, LCA FE, software­system and
databases, Managed LCA content MLC (former GaBi ETAG 018-1
database), University of Stuttgart and Sphera Solutions GmbH, ETAG Nr. 018: GUIDELINE FOR EUROPEAN TECHNICAL
2023 APPROVAL OF FIRE PROTECTIVE PRODUCTS
CUP Version: 2023.1., MLC data set documentation under
https://sphera.com/product­sustainability­gabi­data­search/ EAD 350142-001-1106
(December 2023). EOTA: European Assessment Document: Fire Protective
Products: Fire Protective Board, Slab and Mat Products and
IBU 2021 Kits, 2017
Institut Bauen und Umwelt e.V.: General Instructions for the
EPD programme of Institut Bauen und Umwelt e.V., Version
2.0, Berlin: Institut Bauen und Umwelt e.V., 2021 ETA-17/0170
www.ibu­epd.com ETA­17/ 0170. European Technical Assessment of 28.04.2017.
PCR A
PCR­Part A: Calculation Rules for the Life Cycle Assessment DIN EN 319
and Requirements on the Project Report according to EN DIN EN 319. Particleboards and fibreboards; determination of
15804+A2:2019, Institut Bauen und Umwelt e.V., version 1.3, tensile strength perpendicular to the plane of the board;
2021 German version EN 319:1993
PCR B
PCR– Part B: Requirements of the EPD for Fibre Cement / DIN EN 789
Fibre Concrete, version 8, Institut Bauen und Umwelt e.V., 2023 DIN EN 789. Timber structures ­ Test methods ­ Determination
of mechanical properties of wood based panels; German
version EN 789:2004
96/603/EG und /2000/605/EG
2000/605/EG: Commission Decision of 26 September 2000
amending Decision 96/603/EC establishing the list of products
belonging to Classes A "No contribution to fire" provided for in DIN 4102
Decision 94/611/EC implementing Article 20 of Council DIN 4102­1:1998­05Fire performance of building materials and
Directive 89/106/EEC on construction products. components ­ Part 1: Building Materials; Terms, Requirements
and Tests.
RL 2003/53/EG
Directive 2003/53/EC of the European Parliament and of the
Council of 18 June 2003 amending for the 26th time Council DIN 4108-4:2016– draft
Directive 76/769/EEC relating to restrictions on the marketing DIN 4108­4:2016 – draft, Thermal insulation and energy
and use of certain dangerous substances and preparations economy in buildings ­ Part 4: Hygrothermal design values
(nonylphenol, nonylphenol ethoxylate and cement)
8 Environmental Product Declaration ­ James Hardie Europe GmbH ­ Aestuver® Tx Fire protection board
version EN 13501­2:2008
DIN EN ISO 9001:2015
DIN EN ISO 9001:2015, Quality management systems ­
Requirements (ISO 9001:2015); German and Englisch version Eurofins Umwelt Ost
EN ISO 9001:201 Eurofins Umwelt Ost GmbH, Prüfbericht
AR­24­KS­001439­01 Elemente aus dem 10:1­Schütteleluat
nach DIN EN 12457­4: 2003­01, München, 2024
DIN EN 12467
DIN EN 12467: Fibre­cement flat sheets ­ Product specification
and test methods; German version EN 12467:2012 MPA Eberswalde
MPA Eberswalde Materialprüfanstalt Brandenburg GmbH:
Prüfbericht Nr. 31/24/5372/01, Prüfkammertest (EN
DIN ISO 12572 16516:2017+A1:2020): Bauprodukte – Bewertung der
Hygrothermal performance of building materials and products ­ Freisetzung gefährlicher Stoffe – Bestimmung der Emissionen
Determination of water vapour transmission properties ­ Cup in die Innenraumluft, Eberswalde, 2024
method (ISO 12572:2016); German version EN ISO
12572:2016
MPA NRW.
Materialprüfungsamt Nordrhein­Westfalen: Test report no.
DIN EN 12667 321000741, Aestuver Tx Fire protection board, Determination of
DIN EN 12667 Building materials ­ Determination of thermal natural radioactivity, Dortmund, 2024
resistance by means of guarded hot plate and heat flow meter
methods ­ Dry and moist products with high and medium
thermal resistance. German version EN 12667:2001 Waste codes directory
Ordinance on the European Waste Catalog (Waste Catalog
Ordinance ­ AVV of 10 December 2001, BGBl. I, p.3379, last
DIN EN 13501-2 amended by Article 1 of the Ordinance to Implement the
DIN EN 13501­2. Fire classification of construction products amended Hazardous Waste Criteria of 4 March 2016, BGBl. I p.
and building elements­ Part 2: Classification using data from 382)
fire resistance tests, excluding Ventilation services. German
9 Environmental Product Declaration ­ James Hardie Europe GmbH ­ Aestuver® Tx Fire protection board
Publisher
Institut Bauen und Umwelt e.V. +49 (0)30 3087748­ 0
Hegelplatz 1 info@ibu­epd.com
10117 Berlin www.ibu­epd.com
Germany
Programme holder
Institut Bauen und Umwelt e.V. +49 (0)30 3087748­ 0
Hegelplatz 1 info@ibu­epd.com
10117 Berlin www.ibu­epd.com
Germany
Author of the Life Cycle Assessment
Sphera Solutions GmbH +49711341817­0
Hauptstrasse 111 info@sphera.com
70771 Echterdingen­Leinfelden www.sphera.com
Germany
Owner of the Declaration
James Hardie Europe GmbH 0800 3864001
Bennigsen­Platz 1 Kontakt@jameshardie.de
40474 Düsseldorf www.jameshardie.eu
Germany
10 Environmental Product Declaration ­ James Hardie Europe GmbH ­ Aestuver® Tx Fire protection board
