ENVIRONMENTAL-PRODUCT DECLARATION
as per ISO 14025 and EN 15804+A2
Owner of the Declaration POLYREY
Publisher Institut Bauen und Umwelt e.V. (IBU)
Programme holder Institut Bauen und Umwelt e.V. (IBU)
Declaration number EPD-WIL-20230102-CBA1-EN
Issue date 04/10/2023
Valid to 03/10/2028
Polyrey Nuance wetroom wall panels
Wilsonart
www.ibu-epd.com | https://epd-online.com
1. General Information
Wilsonart Polyrey Nuance wetroom wall panels
Programme holder Owner of the declaration
IBU – Institut Bauen und Umwelt e.V. POLYREY
Hegelplatz 1 Route de Bergerac 700
10117 Berlin 24150 Baneuil
Germany France
Declaration number Declared product / declared unit
EPD-WIL-20230102-CBA1-EN 1 square meter of Nuance panel
This declaration is based on the product category rules: Scope:
Decorative board for interior use, 01/08/2021 The declaration covers a tongue-and-groove system of bathroom and
(PCR checked and approved by the SVR) wetroom wall panels thickness 11,7 mm+/-0,6 mm. The system is named
Polyrey Nuance wetroom wall panels. The declaration covers the total
range of colors. The product is manufactured by WILSONART in its
Issue date Wellingborough plant (UK).
The owner of the declaration shall be liable for the underlying information
04/10/2023
and evidence; the IBU shall not be liable with respect to manufacturer
information, life cycle assessment data and evidences.
Valid to
The EPD was created according to the specifications of EN 15804+A2. In
03/10/2028 the following, the standard will be simplified as EN 15804 bezeichnet.
Verification
The standard EN 15804 serves as the core PCR
Independent verification of the declaration and data according to ISO
14025:2011
internally X externally
Dipl.-Ing Hans Peters
(chairman of Institut Bauen und Umwelt e.V.)
Florian Pronold Dr Naeem Adibi,
(Managing Director Institut Bauen und Umwelt e.V.) (Independent verifier)
1 Environmental-Product Declaration - Wilsonart - Polyrey Nuance wetroom wall panels
2. Product
Performance values of the product are stated in the declaration
2.1 Product description/Product definition of performance, in relation to its essential characteristics
Polyrey Nuance wetroom Wall panels described in the EPD are according to EN438-7:2005 (High-pressure decorative
made from a water-resistant composite material board, glued laminates (HPL) - Sheets based on thermosetting resins
on 2 sides with High Pressure Laminate (HPL), conforming to (Usually called Laminates) - Part 7: Compact laminate and HPL
EN438-3 with a humid-resistant glue. The complete panel composite panels for internal and external wall and ceiling
conforms to EN438-7. The decorative side, made with HPL, finishes)
permits a large range of decors and finishes. The backing side
is made with a balancing HPL. 2.4 Delivery status
Nuance has been treated with Sanitized® – an antibacterial Standard size of panels are:
protection that eliminates 99.9 % of bacteria. 260 × 120 cm rounded edge/tongue
Nuance panel has a rounded edge for optimum finish and 260 × 120 cm tongue/groove
hygiene. The tongue-and-groove assembly system permits 260 × 60 cm tongue/groove
ease of installation and seamless joints. Thickness 11,7 mm +/- 0,6 mm
The final installation is made with Complete adhesive and
Complete colour-matched sealants, ensuring long-term 2.5 Base materials/Ancillary materials
prevention of any water ingress. For the placing on the market The composition of Nuance panels in mass is:
in the European Union/European Free Trade Association . 73 % water-resistant composite board
(EU/EFTA) (except for Switzerland) the Regulation (EU) No . 26 % HPL surface and backing
305/211 applies. The products need a Declaration of . 1 % PUR glue.
Performance taking into consideration EN 438-7, and all have a
CE-marking. The product contains 14 % recycled content from HPL (paper)
and board (PVC) (pre-consumer and post-consumer).
2.2 Application The core is a water-resistant composite board density of 600
Nuance is a patented wall-covering solution suitable for new or kg/m3.
refurbished bathrooms and wetrooms. It can be used instead of The surface and back side are HPL Polyrey conforming to
or on top of existing tiling without having to smooth the surface EN438-3.
down first, or on moisture resistant plasterboard. The gluing is made with water-resistant PUR glue.
2.3 Technical Data The product contains other carcinogenic, mutagenic, reprotoxic
Nuance panels are evaluated according EN438-2 as HPL (CMR) substances of category 1A or 1B that are not on the
bonded board. Detailed information can be found in the candidate list, above 0.1 by weight % in at least one sub-
technical data sheet. product: no.
Constructional data
Biocidal products have been added to this building product or it
Name Value Unit
has been treated with biocidal products (this refers to treated
Gross density 700 kg/m3 goods within the meaning of the Biocidal Products Regulation
Grammage 8.34 kg/m2 (EU) No. 528/2012): yes.
Impact resistance acc. to EN The Sanitized® antibacterial treatment on the Nuance panels is
438-2-21 600 mm free from nanoparticles. It contains a biocide whose active
ingredient is silver phosphate glass which complies with the
Resistance to scratches acc. Min D3 except BRI
Degree REACH and European Biocidal Products regulations (EU) No.
to EN 438-2-25 min D2
528/2012.
Light resistance acc. to EN
4 - 5 -
438-2-27 2.6 Manufacture
Surface adhesion ISO 1. PUR calendar press: gluing of HPL on 2 sides on water-
1 MPa
13894-1-9 resistant composite board with PUR water-resistant glue
Durability - resistance in wet 2. Postforming of HPL for panels with round edge
conditions - 48 h at 40°C EN Mass increase < 8 % 3. Profiling Tongue and groove and edge
438-2-15 modified 4. Unit packaging
The Quality management system is certified: ISO 9001.
Durability - resistance in wet
conditions 48h at 40°C EN >= 4 Degree
2.7 Environment and health during manufacturing
438-2-15 modified
The production conditions do not demand any special health
mm/linear
Flatness EN 438-2-9 <= 3 protection measures over and beyond the legal requirements.
meter
Air: the constitutional valid regulations are observed. The
Height: =/- 1,5 - emissions into the air are below the legally required thresholds.
Dimensional tolerance EN
Width: +/- 1 - mm Water: The process doesn't use or reject water.
438-2-5 and 6
Thickness: +0,4/-0,2 Soil: There is no impact on soil.
mm/linear The Environmental management system is certified: ISO
Squareness EN 438-2-8 <=1,5
meter 14001.
Stain resistance EN 438-2- Group 1&2: 5 -
Grade 2.8 Product processing/Installation
26 Group 3: 4
Nuance panels can be cut using woodworking tools with
Resistance to abrasion EN Taber
150-450 carbide-tipped blades and bits.
438-2-10 rounds
Follow all the usual health and safety precautions when
processing these panels about weight, dust and sharp edges.
2 Environmental-Product Declaration - Wilsonart - Polyrey Nuance wetroom wall panels
Use appropriate personal protective equipment. with a loading factor of 1.0 m2/m3.
The dust produced by processing technical panelling solutions This is in line with the current state of knowledge.
may irritate the skin or lungs, so use a dust collector whenever
cutting wood and wear appropriate personal protective 2.12 Reference service life
equipment. The estimated service life of Nuance panel depends on the
The assembly of the panels is done by gluing with Complete area of application (private or commercial use), the users
adhesive. themselves and the maintenance of the product. According to
For new builds, the panels can be bonded directly on moisture- the Federal Office for Building and Regional Planning (BBSR) a
resistant plasterboard by waterproofing the substrate and reference service life of 20 years can be assumed for
applying a primer. laminate/plastic coverings. The use stage (module B2) is
For renovation, the panels can be bonded directly on tiling or declared in this EPD for 20 years of usage assuming 50 %
paintwork after carefully checking and waterproofing the domestic and 50 % commercial level of use.
substrate and sealing treatment.
2.13 Extraordinary effects
The correct preparation of the substrate (flatness,
waterproofing...) is key and detailed in the processing brochure. Fire
The assembly is done thanks to the tongue and groove system Nuance panels are classified as E according to EN13501-1 and
and the coloured connection joint Complete provides a M3 according to NFP 92-501.
seamless joint. Water
Detailed information and processing are available at Nuance panels are designed for use in an interior fitting of
www.polyrey.com bathrooms or wetroom walls.
When installed according to the technical guideline and using
2.9 Packaging Complete adhesives and sealants, the water doesn't have any
Nuance panels are delivered unit-packed, and edge-protected impact on the Nuance system.
using cardboard. No substances that can be hazardous to water are washed out.
Cardboard can be recycled materially or energetically.
Pallets are used for the delivery. The pallets can be reused. Mechanical destruction
The surface of HPL of Nuance panels gives good performance
2.10 Condition of use regarding impact, according to EN 438-3 specification. The
The composition during the use phase refers to the composition application of Nuance panels is a vertical application for wall
during the manufacturing. panelling in bathrooms and wetrooms therefore not subject to
Core and HPL panels are chemically inert and the bonding strong mechanical aggression.
agents are chemically stable and permanently bonded to the Moreover in case of severe damage the damaged panels
core. should be replaced.
No hazardous substances are released during mechanical
2.11 Environment and health during use destruction.
Environmental protection:
When the described products are used properly in accordance 2.14 Re-use phase
with the area of application, there is no risk of water, air, or Currently, there is no possible re-use or recycling option. The
ground contamination according to the current state of scenario for the end of life is a landfill.
knowledge.
2.15 Disposal
Health protection: Waste from Nuance panels is classed according to the
When used normally and in accordance with the intended European Waste Catalogue under the six-digit waste code 20
purpose, no health risks or restrictions are to be anticipated 03 01. It is defined as «mixed municipal waste» which can be
with Nuance panels. disposed of as household or commercial waste.
Except for minor amounts of formaldehyde in quantities that are
2.16 Further information
harmless to health, no emissions of hazardous substances can
be detected. Detailed information and recommendations are available on
VOC emissions are measured for A ratings in tests on walls www.polyrey.com
3. LCA: Calculation rules
• Production of pre-products, extraction of energy
3.1 Declared Unit
carriers, raw material transportation, manufacture of
This declaration refers to the declared unit of 1 m² of Nuance
product and packaging materials are declared in
board. The weight of the product is 8.34 kg/m².
modules A1-A3.
Declared unit and mass reference Modules A1-A3 also include the manufacturing and
Name Value Unit supply of energy.
Declared unit 1 m2 • The scenario for the transport of the product to the
construction site is declared in module A4.
Grammage 8.34 kg/m2
• The treatment of packaging materials at installation,
Layer thickness 0.0117 m installation auxiliaries as well as installation losses are
declared in module A5.
• The use stage includes emissions occurring during the
3.2 System boundary lifetime of the product (B1) as well as the maintenance
The type of EPD is cradle to gate with options. The additional stage/cleaning (B2).
modules are modules A4, A5, B1 and B2. • Two end-of-life scenarios are declared in the EPD. They
include manual dismantling (C1), transportation to waste
Considered product stages: processing (C2),
3 Environmental-Product Declaration - Wilsonart - Polyrey Nuance wetroom wall panels
• Scenario 1: 100 % thermal treatment with energy Where country/region-specific data are
recovery (C3/1). Credits for electricity and thermal unavailable, proxy data are used. The overall
energy, which result from energy recovery in modules geographical representativeness is
A5 and C3, are declared in module D/1. considered to be good.
• Scenario 2: 100 % landfilling (C4/2). Credits for • All primary and secondary data are modelled
electricity and thermal energy, which result from energy to be specific to the technologies or
recovery in module A5, are declared in module D/2. technology mixes under study. Where
• The CO incorporation in the product (from the technology-specific data is unavailable,
2
sequestration in the paper material) is proxy data are used. The overall
considered. The C-balance is closed by considering the technological representativeness is
biotic CO emissions according to the incorporation on considered to be good.
2
• Primary data are collected by the client using
the input side.
a specifically adapted spreadsheet. Sphera
3.3 Estimates and assumptions supported the data collection by preparing a
The following assumptions are included in the EPD: specific questionnaire and virtual or onsite
support.
• It is assumed that packaging materials are disposed of
Overall, the data quality can be described as good.
via incineration (wooden pallets) and recycling
The primary data collection has been done thoroughly;
(cardboard).
all relevant flows are considered.
• Distance to the end of life of non-hazardous waste is
assumed as 50km. 3.7 Period under review
The period under review for the collection of production
3.4 Cut-off criteria
data is the year 2021.
The packaging of the raw materials, as well as their disposal, is
not considered in the scope of this study. 3.8 Geographic Representativeness
Transportation of installation auxiliaries' materials is also not Land or region, in which the declared product system is
considered in the scope of this study. manufactured, used or handled at the end of the product´s
lifespan: Europe
3.5 Background data
The background data has been taken from the latest
available GaBi database CUP 2022.1. The 3.9 Allocation
requirements for data quality and background data The production process does not deliver any co-products. The
correspond to the specifications of the PCR Part A. applied software model does not contain any allocation.
3.6 Data quality
The overall production of Wilsonart comprises further products
The requirements on the data quality and the
besides the products considered in this study. Data for electrical
background data correspond to the provisions in EN
energy refers to the declared product. During data collection,
15804 and the IBU PCR part A (IBU 2020)
the
respectively:
allocation is done via quantities (mass) produced.
3.10 Comparability
• All primary data are collected for the year
2021. All secondary data come from the GaBi Basically, a comparison or an evaluation of EPD data is only
databases and are representative of the years possible if all the data sets to be compared were created
2017-2022. As the study intended to compare the according to EN 15804 and the building context, respectively
product systems for the reference year the product-specific characteristics of performance, are taken
2021, temporal representativeness is good. into account. Background dataset: GaBi ts software, CUP
• All primary and secondary data are collected 2022.1.
specific to the countries/regions under study.
4. LCA: Scenarios and additional technical information
Characteristic product properties
Transport to the building site (A4)
Information on biogenic carbon
Module A4 considers a 600 km truck transport from the
manufacturing plant in the UK to an average European
Biogenic carbon is present in the product and the packaging
customer site.
materials.
Name Value Unit
Note: 1 kg biogenic Carbon is equivalent to 44/12 kg of CO Litres of fuel (truck Euro 6) 0.013 l/100km
2
Transport distance 600 km
Information on describing the biogenic Carbon Content at
factory gate Capacity utilisation (including empty runs) 61 %
Name ValueUnit
Installation into the building (A5)
kg
Biogenic carbon content in product 0.66 The installation of the Nuance board is done manually with
C
some electric tools (e.g. cutting saw). Adhesive and sealant are
Biogenic carbon content in accompanying kg needed for the installation.
0.66
packaging C
Installation losses have been accounted for in module A5.
Product losses have been considered as 15 %. Losses are
The following technical information is a basis for the declared
disposed of in a landfill.
modules.
The packaging material treatment and disposal are also
4 Environmental-Product Declaration - Wilsonart - Polyrey Nuance wetroom wall panels
considered in module A5. themselves and the maintenance of the product. According to
Name ValueUnit BBSR a reference service life of 20 years can be assumed for
laminate/plastic coverings. The use stage (module B2) is
Auxiliary (adhesive and sealant) 0.18 kg
declared in this EPD for 20 years of usage assuming 50 %
Electricity consumption (for cutting) 0.06 kWh
domestic and 50 % commercial level of use.
Material loss (15 %) 1.25 kg
Reference service life
Output substances following waste treatment on
1.605 kg Name Value Unit
site (packaging materials)
Life Span according to the manufacturer 20 a
Packaging material:
Cardboard: 0,105 kg/m² End of life (C1-C4)
Wood pallets: 1,5 kg/m² The deconstruction (module C1) is assumed to be done
manually (no environmental impact).
Use (B1)
Emissions to air occur during the use stage of the product. The The transport to waste processing (module C2) is assumed to
following emissions are considered in module B1. be 50 km.
Name Value Unit
Scenario 1 : Thermal treatment with energy recovery (C3/1)
Formaldehyde emissions (for the RSL) 1,60E-08 kg/m²
Scenario 2 : Landfilling (C4/2)
VOC emissions (for the RSL) 7,5E-09 kg/m²
Name Value Unit
Maintenance (B2) Collected as mixed construction waste 8.34 kg
Module B2 includes the cleaning of the board. Water and Landfilling (Scenario 1) 8.34 kg
detergent are required for the cleaning. The scenario considers Energy recovery (Scenario 2) 8.34 kg
installation in the following conditions: 50 % residential (1
cleaning/week) and 50 % hotel (1 cleaning/day - 70 % load).
Reuse, recovery and/or recycling potentials (D)
This results in 154 cleanings per year. The following table
Module D/1 includes the potential benefits in form of energy
documents the water and auxiliaries consumption for the
recovery of the incineration process in A5 (incineration of
cleaning of 1 m² per year.
packaging wastes) and C4 (combustion of the product).
Name Value Unit
Water consumption 0.0077 m3 Module D/2 includes the potential benefits in form of energy
Auxiliary (detergent) 0.123 kg recovery of the incineration process in A5 (incineration of
packaging wastes).
The estimated service life of Nuance panels depends on the
area of application (private or commercial use), the users
5 Environmental-Product Declaration - Wilsonart - Polyrey Nuance wetroom wall panels
5. LCA: Results
The following tables display the environmentally relevant results according to EN 15804+A2 for 1 m² Nuance board.
Two end-of-life scenarios are declared in the EPD:
C3/1: 100 % thermal treatment of the product with energy recovery
D/1: benefits in form of energy recovery of the incineration process in A5 (incineration of packaging wastes) and C4 (combustion of the
product).
C4/2: 100 % landfilling
D/2: benefits in form of energy recovery of the incineration process in A5 (incineration of packaging wastes).
DESCRIPTION OF THE SYSTEM BOUNDARY (X = INCLUDED IN LCA; ND = MODULE OR INDICATOR NOT DECLARED; MNR =
MODULE NOT RELEVANT)
BENEFITS
AND LOADS
CONSTRUCTION
BEYOND
PRODUCT STAGE PROCESS USE STAGE END OF LIFE STAGE
THE SYSTEM
STAGE
BOUNDARIE
S
la ire ta m w a Ry lp p u s tro p s n a rT g n iru tc a fu n a M e h t m o rf tro p s n a rTe tis e h t o t e ta g y lb m e s s A e s U e c n a n e tn ia M ria p e R tn e m e c a lp e R tn e m h s ib ru fe R y g re n e la n o ita re p Oe s u re ta w la n o ita re p Oe s u n o itc u rts n o c -e Dn o itilo m e d tro p s n a rT g n is s e c o rp e ts a W la s o p s iD -e s u e R-y re v o c e R-g n ilc y c e Rla itn e to p
A1 A2 A3 A4 A5 B1 B2 B3 B4 B5 B6 B7 C1 C2 C3 C4 D
X X X X X X X MNR MNR MNR MND MND X X X X X
RESULTS OF THE LCA - ENVIRONMENTAL IMPACT according to EN 15804+A2: 1 m² Nuance board
Parameter Unit A1-A3 A4 A5 B1 B2 C1 C2 C3/1 C3/2 C4/1 C4/2 D/1 D/2
GWP-total kg CO 2 eq 4.3E+01 4.55E-01 1.23E+01 0 1.96E+00 0 3.25E-02 1.84E+01 0 0 5.39E+00 -5.02E+00 -9.51E-01
GWP-fossil kg CO 2 eq 4.77E+01 4.5E-01 1.02E+01 0 1.87E+00 0 3.22E-02 1.6E+01 0 0 2.7E-01 -4.81E+00 -7.58E-01
GWP-
biogenic kg CO 2 eq -4.75E+00 1.89E-03 2.05E+00 0 9.48E-02 0 1.35E-04 2.42E+00 0 0 5.11E+00 -2.11E-01 -1.93E-01
GWP-luluc kg CO 2 eq 3.36E-02 3.09E-03 5.82E-03 0 1.12E-03 0 2.2E-04 1.25E-03 0 0 2.51E-04 -5.06E-04 -8.02E-05
kg CFC11
ODP 2.48E-09 4.5E-14 3.77E-10 0 5.21E-13 0 3.21E-15 1.57E-11 0 0 4.41E-13 -3.5E-11 -5.55E-12
eq
AP mol H+ eq 1.56E-01 5.12E-04 2.54E-02 0 8.4E-03 0 3.65E-05 5E-03 0 0 1.67E-03 -6.11E-03 -9.66E-04
EP-
kg P eq 1.17E-04 1.64E-06 1.94E-05 0 1.04E-04 0 1.17E-07 4.02E-06 0 0 7.69E-06 -6.98E-06 -1.11E-06
freshwater
EP-marine kg N eq 4.08E-02 1.65E-04 6.72E-03 0 1.77E-03 0 1.18E-05 1.67E-03 0 0 6.01E-04 -1.6E-03 -2.52E-04
EP-terrestrial mol N eq 4.19E-01 1.97E-03 7.02E-02 0 1.53E-02 0 1.41E-04 2.08E-02 0 0 5.78E-03 -1.7E-02 -2.69E-03
kg NMVOC
POCP 1.14E-01 4.41E-04 1.97E-02 2.15E-08 4.98E-03 0 3.15E-05 4.75E-03 0 0 3.04E-03 -4.34E-03 -6.85E-04
eq
ADPE kg Sb eq 2.31E-05 4.62E-08 3.97E-06 0 3.67E-06 0 3.3E-09 3.85E-07 0 0 2.1E-08 -6.52E-07 -1.03E-07
ADPF MJ 6.61E+02 6.01E+00 1.19E+02 0 5.11E+01 0 4.29E-01 2.95E+01 0 0 3.58E+00 -4.34E+01 -6.88E+00
m3 world
WDP eq 6.7E+00 5.13E-03 1.51E+00 0 6.34E-01 0 3.66E-04 1.65E+00 0 0 2.94E-02 -5.45E-01 -8.65E-02
deprived
GWP = Global warming potential; ODP = Depletion potential of the stratospheric ozone layer; AP = Acidification potential of land and water; EP =
Eutrophication potential; POCP = Formation potential of tropospheric ozone photochemical oxidants; ADPE = Abiotic depletion potential for non-fossil
resources; ADPF = Abiotic depletion potential for fossil resources; WDP = Water (user) deprivation potential)
RESULTS OF THE LCA - INDICATORS TO DESCRIBE RESOURCE USE according to EN 15804+A2: 1 m² Nuance board
Parameter Unit A1-A3 A4 A5 B1 B2 C1 C2 C3/1 C3/2 C4/1 C4/2 D/1 D/2
PERE MJ 1.34E+02 4.17E-01 5.3E+01 0 1.85E+00 0 2.98E-02 2.72E+01 0 0 3.76E-01 -2.41E+01 -3.82E+00
PERM MJ 4.35E+01 0 -2.4E+01 0 0 0 0 -1.94E+01 0 0 0 0 0
PERT MJ 1.78E+02 4.17E-01 2.89E+01 0 1.85E+00 0 2.98E-02 7.81E+00 0 0 3.76E-01 -2.41E+01 -3.82E+00
PENRE MJ 5.68E+02 6.04E+00 1.19E+02 0 5.11E+01 0 4.31E-01 1.23E+02 0 0 3.58E+00 -4.34E+01 -6.88E+00
PENRM MJ 9.36E+01 0 0 0 0 0 0 -9.36E+01 0 0 0 0 0
PENRT MJ 6.61E+02 6.04E+00 1.19E+02 0 5.11E+01 0 4.31E-01 2.95E+01 0 0 3.58E+00 -4.34E+01 -6.88E+00
SM kg 1.28E+00 0 1.92E-01 0 0 0 0 0 0 0 0 0 0
RSF MJ 0 0 0 0 0 0 0 0 0 0 0 0 0
NRSF MJ 0 0 0 0 0 0 0 0 0 0 0 0 0
FW m3 1.98E-01 4.82E-04 4.39E-02 0 1.49E-02 0 3.44E-05 4.2E-02 0 0 8.26E-04 -2.3E-02 -3.64E-03
PERE = Use of renewable primary energy excluding renewable primary energy resources used as raw materials; PERM = Use of renewable primary
energy resources used as raw materials; PERT = Total use of renewable primary energy resources; PENRE = Use of non-renewable primary energy
excluding non-renewable primary energy resources used as raw materials; PENRM = Use of non-renewable primary energy resources used as raw
materials; PENRT = Total use of non-renewable primary energy resources; SM = Use of secondary material; RSF = Use of renewable secondary fuels;
6 Environmental-Product Declaration - Wilsonart - Polyrey Nuance wetroom wall panels
NRSF = Use of non-renewable secondary fuels; FW = Use of net fresh water
RESULTS OF THE LCA – WASTE CATEGORIES AND OUTPUT FLOWS according to EN 15804+A2:
1 m² Nuance board
Parameter Unit A1-A3 A4 A5 B1 B2 C1 C2 C3/1 C3/2 C4/1 C4/2 D/1 D/2
HWD kg 1.86E-05 3.19E-11 2.79E-06 0 1.7E-04 0 2.28E-12 2.31E-09 0 0 4.28E-10 -3.76E-09 -5.95E-10
NHWD kg 7.77E-01 9.84E-04 1.63E+00 0 1.62E-01 0 7.02E-05 9.9E+00 0 0 8.52E+00 -3.27E-02 -5.18E-03
RWD kg 2.21E-02 1.12E-05 3.67E-03 0 7.93E-04 0 8E-07 9.53E-04 0 0 4.26E-05 -6.94E-03 -1.1E-03
CRU kg 0 0 0 0 0 0 0 0 0 0 0 0 0
MFR kg 1.22E-02 0 1.07E-01 0 0 0 0 0 0 0 0 0 0
MER kg 0 0 0 0 0 0 0 0 0 0 0 0 0
EEE MJ 0 0 5.78E+00 0 0 0 0 1.71E+01 0 0 0 0 0
EET MJ 0 0 1.04E+01 0 0 0 0 3.11E+01 0 0 0 0 0
HWD = Hazardous waste disposed; NHWD = Non-hazardous waste disposed; RWD = Radioactive waste disposed; CRU = Components for re-use;
MFR = Materials for recycling; MER = Materials for energy recovery; EEE = Exported electrical energy; EET = Exported thermal energy
RESULTS OF THE LCA – additional impact categories according to EN 15804+A2-optional:
1 m² Nuance board
Parameter Unit A1-A3 A4 A5 B1 B2 C1 C2 C3/1 C3/2 C4/1 C4/2 D/1 D/2
Disease
PM 2.64E-06 3.52E-09 4.21E-07 0 6.24E-08 0 2.51E-10 1.1E-07 0 0 1.78E-08 -4.96E-08 -7.85E-09
incidence
kBq U235
IR 2.24E+00 1.69E-03 3.8E-01 0 1.3E-01 0 1.21E-04 1.08E-01 0 0 5.8E-03 -1.18E+00 -1.86E-01
eq
ETP-fw CTUe 2.07E+02 4.26E+00 4.33E+01 2.94E-06 7.32E+01 0 3.04E-01 2.44E+01 0 0 1.75E+00 -1.9E+01 -3.01E+00
HTP-c CTUh 7.17E-08 8.78E-11 1.13E-08 2.11E-13 9.85E-10 0 6.27E-12 9.78E-10 0 0 2.07E-10 -7.66E-10 -1.21E-10
HTP-nc CTUh 9.07E-06 4.77E-09 1.41E-06 3.08E-15 7.73E-08 0 3.4E-10 1.03E-07 0 0 2.59E-08 -2.07E-08 -3.28E-09
SQP SQP 8.86E+02 2.55E+00 1.36E+02 0 9.97E-01 0 1.82E-01 6.81E+00 0 0 4.21E-01 -1.56E+01 -2.48E+00
PM = Potential incidence of disease due to PM emissions; IR = Potential Human exposure efficiency relative to U235; ETP-fw = Potential comparative
Toxic Unit for ecosystems; HTP-c = Potential comparative Toxic Unit for humans (cancerogenic); HTP-nc = Potential comparative Toxic Unit for humans
(not cancerogenic); SQP = Potential soil quality index
Disclaimer 1 – for the indicator 'Potential Human exposure efficiency relative to U235'.This impact category deals mainly with the
eventual impact of low-dose ionizing radiation on human health of the nuclear fuel cycle. It does not consider effects due to possible
nuclear accidents, occupational exposure or radioactive waste disposal in underground facilities. Potential ionizing radiation from the
soil, radon and from some construction materials is also not measured by this indicator.
Disclaimer 2 – for the indicators 'abiotic depletion potential for non-fossil resources', 'abiotic depletion potential for fossil resources',
'water (user) deprivation potential, deprivation-weighted water consumption', 'potential comparative toxic unit for ecosystems', 'potential
comparative toxic unit for humans – cancerogenic', 'Potential comparative toxic unit for humans - not cancerogenic', 'potential soil
quality index'. The results of this environmental impact indicator shall be used with care as the uncertainties on these results are high
as there is limited experience with the indicator.
6. LCA: Interpretation
The interpretation is based on the assumptions and limitations potential.
described in the background report, both with regard to the
methods and the data. A dominance analysis is used for
interpretation. The following figure shows the results of the
individual modules as an example of the global warming
It is visible that the manufacturing phase dominates the product
system. In addition, the packaging treatment in module A5 has
7 Environmental-Product Declaration - Wilsonart - Polyrey Nuance wetroom wall panels
relevant environmental impacts.
• Production of the composite board (a major component
of the Nuance product) has a significant influence (>50
The C3/1 module (incineration scenario) is the second highest
%) on nearly all indicators. It represents more than 75 %
contributor to the GWP impact, due to combustion emissions.
of the impacts in the GWP-total, ODP, ADPE and water
The GWP impact in the C4/2 module (landfilling scenario) is
use indicators.
mostly due to the release of the biogenic carbon stored in the
• The GWP-biogenic is shared by the HPL production and
HPL as both carbon dioxide and methane. Results for module
the packaging materials (wood pallets and cardboard)
B2 are declared for the RSL of 20 years.
due to the carbon sequestered in the materials.
• Transportation of raw materials has a relevant influence
(between 25 % and 50 %) to the AP, EP-marine, EP-
Interpretation of results for the environmental indicators
terrestrial and POCP indicators.
according to ISO 14044:
• The production process and energy consumption
comparatively have minor impacts overall.
7. Requisite evidence
ISO 16000 are empirically and theoretically analysed.
AgBB overview of results (28 days [µg/m³])
VOC and formaldehyde emissions
Name Value Unit
Determination of the VOC and formaldehyde emission
according to/compliance with AgBB-Scheme / ISO 16000 part TVOC (C6 - C16) 10 μg/m3
3, 6 and 9 Sum SVOC (C16 - C22) < 5 μg/m3
R (dimensionless) 170 -
Measurement centre: Eurofins Product Testing A/S-
VOC without NIK < 5 μg/m3
Smedeskovvej 38 -8464 Galten - Denmark
Carcinogenic Substances < 1 μg/m3
Test report: 392-2019-00131801-A-EN-03 of 02.04.2019 Formaldehyde 16 µg/m3
Result: AgBB overview of results (3 days [µg/m³])
A rating according to the regulation of March and May 2011 - Name Value Unit
tested according to a wall scenario with a loading factor of 1.0
TVOC (C6 - C16) 20 μg/m3
m2/m3
Sum SVOC (C16 - C22) < 5 μg/m3
Formaldehyde E1 class - formaldehyde result based on
chamber testing and DNPH sampling according to ISO 16000. R (dimensionless) 250 -
The result is therefore not directly according to EN 717-1, and VOC without NIK < 5 μg/m3
there are a few small deviations. The testing is in accordance
Carcinogenic Substances < 1 μg/m3
with the conclusions presented in CEN TC351 WG2 N174
where the difference and compatibility between EN 717-1 and
8. References
Standards ISO 9001
ISO 9001: 2015: Quality Management System
EN 438 : High-pressure decorative laminates (HPL) -
Sheets based on thermosetting resins (usually called ISO 13894
laminates) ISO 13894 : High-pressure decorative laminate - Composite
EN438-2:2016 : Part 2: Determination of properties elements - Part 1 : test methods - part 2 : specifications
EN438-3:2016: Part 3 : classification and specifications for
laminates less than 2 mm thick intended for bonding to ISO 14001
supporting substrates ISO 14001: 2015: Environmental Management System
EN438-7 : 2005 :Part 7: Compact laminate and HPL composite
panels for internal and external wall and ceiling finishes ISO 14025
EN ISO 14025:2011, Environmental labels and declarations —
EN 717-1 Type III environmental
EN 717-1: 2004:Wood-based panels. Determination of declarations — Principles and procedures.
formaldehyde release Formaldehyde emission by the chamber
method ISO 16000
ISO 16000: Indoor air - Part 3 : determination of formaldehyde -
Part 6 :
EN 13501-1 determination of organic compounds - Part 9 : determination of
EN13501-1: Fire classification of construction products and the
building elements - emission of volatile organic compounds from building products
Part 1 : classification using data from reaction to fire tests and
furnishing - Emission test chamber method
EN 15804
EN15804:2012+A2:2019+AC:2021, Sustainability of NFP 92-501
construction works —Environmental Product Declarations — NFP 92-501 : Safety against fire - Building materials - Reaction
Core rules for the product category of construction products. to fire tests
8 Environmental-Product Declaration - Wilsonart - Polyrey Nuance wetroom wall panels
Further References IBU 2021
Institut Bauen und Umwelt e.V.: General Instructions for the
BBSR EPD programme of Institut
BBSR table (german): 'Nutzungsdauern von Bauteilen zur Bauen und Umwelt e.V., Version 2.0, Berlin: Institut Bauen und
Lebenszyklusanalyse nach Umwelt e.V., 2021 www.ibu-epd.com
BNB', Bundesinstitut für Bau-, Stadt- und Raumforschung,
Referat II Nachhaltiges Bauen; online available under PCR Part A
https://www.nachhaltigesbauen.de/austausch/nutzungsdauernvon- PCR - Part A: Calculation rules for the Life Cycle Assessment
auteilen/ and Requirements on the
Background Report, version 1.6, Institut Bauen und Umwelt
e.V.,
www.bau-umwelt.com, 2017
BPR
BPR : Biocidal Products PCR Part B
Regulation (BPR) refers to Regulation (EU) 528/2012 Part B: Requirements on the EPD for Decorative board for
concerning the interior use , 09/2022
placing on the market and use of biocidal products.
REACH
GaBi Regulation (EC) No 1907/2006 concerning the Registration,
GaBi Software System and Database for Life Cycle Evaluation, Authorisation and
Engineering, 1992-2021, Sphera Restriction of Chemicals (REACH)
Solutions GmbH, Leinfelden-Echterdingen, with
acknowledgement of LBP University Regulation (EU) No 305/2011
of Stuttgart, program version GaBi 10; database version 2022.1 Regulation (EU) No 305/2011 of the European Parliament and
of the Council of 9 March 2011 laying down harmonised
GaBi documentation conditions for the marketing of construction products and
GaBi dataset documentation for the software system and repealing Council Directive 89/106/EEC
databases, LBP, University of
Stuttgart and Sphera Solutions GmbH, Leinfelden- European Waste Catalogue
Echterdingen, 2021. Guidance on Classification of Waste according to EWC-stat
(http://www.gabi-software.com/support/gabi/gabi[1]database- categories version 2, December 2010
2021-lci-documentation/)
9 Environmental-Product Declaration - Wilsonart - Polyrey Nuance wetroom wall panels
Publisher
Institut Bauen und Umwelt e.V. +49 (0)30 3087748- 0
Hegelplatz 1 info@ibu-epd.com
10117 Berlin www.ibu-epd.com
Germany
Programme holder
Institut Bauen und Umwelt e.V. +49 (0)30 3087748- 0
Hegelplatz 1 info@ibu-epd.com
10117 Berlin www.ibu-epd.com
Germany
Author of the Life Cycle Assessment
Sphera Solutions GmbH +49 711 341817-0
Hauptstraße 111- 113 info@sphera.com
70771 Leinfelden-Echterdingen www.sphera.com
Germany
Owner of the Declaration
POLYREY +33 (0)5 53 63 80 80
Route de Bergerac 700 support.technique@polyrey.com
24150 Baneuil www.polyrey.com
France
10 Environmental-Product Declaration - Wilsonart - Polyrey Nuance wetroom wall panels
