ENVIRONMENTAL
as per ISO 14025 and EN 15804+A2
Owner of the Declaration modulyss®
Programme holder Institut Bauen und Umwelt e.V. (IBU)
Publisher Institut Bauen und Umwelt e.V. (IBU)
Declaration number EPD-MOD-20220309-CBA1-EN
Issue date 10.01.2023
Valid to 09.01.2028
Modular carpet tiles
Pile material: polyamide 6 yarn with a maximum total pile
weight of 1300 g/m2
Back2Back or Comfortback
modulyss®
www.ibu-epd.com | https://epd-online.com
Umwelt Produktdeklaration Name des Herstellers – Name des Produkts
General Information
modulyss® Modular carpet tiles
pile material: polyamide 6 yarn with a
maximum total pile weight of 1300
g/m2
Back2Back or Comfortback
Programme holder Owner of the declaration
IBU – Institut Bauen und Umwelt e.V. modulyss
Hegelplatz 1 Zevensterrestraat 21
10117 Berlin 9240 Zele
Germany Belgium
Declaration number Declared product / declared unit
EPD-MOD-20220309-CBA1-EN 1 m² tufted modular carpet tiles with bitumen heavy
backing and a pile material of PA 6
This declaration is based on the product Scope:
category rules: The manufacturer declaration applies to tufted carpet
Floor coverings, 02/2018 tiles with bitumen heavy backing, a pile material of PA
(PCR checked and approved by the SVR) 6 with a maximum total pile weight of 1300 g/m2. The
products are produced in Zele, Belgium.
LCA results for products with a maximum total pile
Issue date
weight of 480 g/m2 can be taken from the
10.01.2023
corresponding tables of the annexe. Specific data for
every product within the declared group of products in
Valid to relation to its total pile weight can be calculated by
09.01.2028 using equation 1 given in the annexe (see annexe
chapter: 'General Information on the annexe'). The
declaration is only valid in conjunction with a valid
GUT-PRODIS license of the product.
The owner of the declaration shall be liable for the
underlying information and evidence; the IBU shall not
be liable with respect to manufacturer information, life
cycle assessment data and evidences.
The EPD was created according to the specifications
of EN 15804+A2. In the following, the standard will be
simplified as EN 15804.
Verification
The standard EN 15804 serves as the core PCR
Independent verification of the declaration and data
according to ISO 14025:2011
Dipl. Ing. Hans Peters internally x externally
(chairman of Institut Bauen und Umwelt e.V.)
Dr. Alexander Röder Angela Schindler
(Managing Director Institut Bauen und Umwelt e.V.)) (Independent verifier)
Product
Product description/Product definition For the placing on the market of the specific product in
The declaration applies to tufted carpet tiles having a the European Union/European Free Trade Association
surface pile of polyamide 6 with a maximum total pile (EU/EFTA) (with the exception of Switzerland)
weight of 1300 g/m2. Colouring of the surface is Regulation (EU) No. 305/2011 Construction Product
achieved using either solution-dyed yarn or aqueous Regulation (CPR) applies. The product needs a
dyeing methods. The backing of the carpet consists of Declaration of Performance (DoP) taking into
a bitumen heavy backing. In the comfortback range, consideration EN 14041:2018-05, Resilient, textile and
the bitumen heavy backing is covered by a PET fleece. laminate floor coverings - Essential characteristics, and
The total recycled content of the carpet is 49 %. the CE-marking. The DoP of the product can be found
on the manufacturer's technical information section.
2 Environmental Product Declaration modulyss – Tufted tiles, polyamide 6 with a maximum total pile weight of 1300 g/m2,
back2back or comfortback
For the application and use of the product the Styrene butadiene rubber (SBR) 4.8 %
respective national provisions apply. SBS Copolymer 1.1 %
Bitumen 11.3 %
Application Glass fibre 0.2 %
The use class of the specific product as defined in Additives 0.9 %
EN 1307 can be found in the Product Information
System (PRODIS) using the PRODIS registration The specific product covered by the EPD contains
number of the product. substances listed in the ECHA candidate list
(08.07.2021) or other carcinogenic, mutagenic or
Technical Data
reprotoxic (CMR) substances in categories 1A or 1B
which are not on the candidate list exceeding 0.1
percentage by mass: no
Constructional data according to EN 1307 The products are registered in the GUT-PRODIS
Name Value Unit Information System. The GUT-PRODIS system
Modular carpet tiles, 50 cm x
Product Form - ensures compliance with limitations of various
50 cm
chemicals and Volatile Organic Compound s(VOC)-
Type of manufacture Tufted carpet - emissions and a ban on the use of all substances that
Yarn type Polyamide 6 - are listed as 'Substances of Very High Concern'
Total carpet weight 5277 g/m2 (SVHC) under REACH.
Bitumen heavy backing with
Secondary backing -
textile bottom Reference service life
The service life of textile floor coverings strongly
depends on the correct installation taking into account
Performance data of the product in accordance with the declared use classification and the adherence to
the declaration of performance with respect to its cleaning and maintenance instructions.
essential characteristics according to EN 14041: 2018- A calculation of the reference service life according to
05, Resilient, textile and laminate floor coverings - ISO 15686 is not possible.
Essential characteristics. Alternatively, a reference service life of 10 years can
Additional product properties in accordance with EN be assumed, during which the functional and visual
1307 can be found on the Product Information System quality is guaranteed (BNB, Nutzungsdauer von
PRODIS using the PRODIS registration number of the Bauteilen). The technical service life can be
product (www.pro-dis.info) or on the manufacturer's significantly longer.
technical information section.
Base materials/Ancillary materials
Name Value Unit
Polyamide 6 24.6 %
Polypropylene 0.6 %
Polyester 10.2 %
Limestone 41.0 %
Aluminiumhydroxide 5.3 %
LCA: Calculation rules
Declared Unit 1 - landfill disposal
2 - municipal waste incineration
3 - recovery in a cement plant
Name Value Unit
Declared unit 1 m2 A1-A3 Production:
Grammage 5277 kg/m2 Energy supply and production of the basic material,
The declared unit refers to 1 m2 produced textile floor processing of secondary material, auxiliary material,
covering. The output of module A5 'Assembly' is 1 m2 transport of the material to the manufacturing site,
installed textile floor covering. emissions, waste water treatment, packaging material
The layer thickness of the specific product covered by and waste processing up to the landfill disposal of
the EPD can be found on the Product Information residual waste (except radioactive waste). Benefits for
System PRODIS using the PRODIS registration generated electricity and steam due to the incineration
number of the product (www.pro-dis.info) or on the of production waste are aggregated.
manufacturer's technical information section. Biogenic carbon that is stored in renewable material
(wood resin, renewable additives, packaging paper) is
taken into account as well as the associated carbon
dioxide uptake from the air from which this biogenic
System boundary carbon comes.
Type of EPD: Cradle-to-gate with options A4 Transport:
System boundaries of modules A, B, C, D: Transport of the packed textile floor covering
Modules C3, C4 and D are indicated separately for from factory gate to the place of installation.
three end-of-life scenarios:
3 Environmental Product Declaration modulyss – Tufted tiles, polyamide 6 with a maximum total pile weight of 1300 g/m2,
back2back or comfortback
A5 Installation: C2 Transport:
Installation of the textile floor covering, processing of Transport of the carpet waste to a landfill, to the
installation waste and packaging waste up to the municipal waste incineration plant (MWI) or to the
landfill disposal of residual waste (except radioactive waste collection facility for recycling.
waste), the production of the amount of carpet that
occurs as installation waste including its transport to C3 Waste processing:
the place of installation. C3-1: Landfill disposal needs no waste processing.
Generated electricity and steam due to the incineration C3-2: Impact from waste incineration (plant with R1 >
of waste are listed in the result table as exported 0.6), generated electricity and steam are listed in the
energy. result table as exported energy.
Biogenic carbon that is stored in renewable materials C3-3: Collection of the carpet waste for recovery in the
in installation waste and packaging paper is released cement industry, waste processing (granulating),
as carbon dioxide emissions into the air at the end of transport to the cement plant, emissions from the
life in module A5. incineration.
Preparation of the floor and auxiliary materials
(adhesives, fixing agents, PET connectors) are beyond C4 Disposal
the system boundaries and not taken into account. C4-1: Impact from landfill disposal,
C4-2: The carpet waste leaves the system in module
B1 Use: C3-2,
Indoor emissions during the use stage. After the first C4-3: The pre-processed carpet waste leaves the
year, no product-related Volatile Organic Compound system in module C3-3.
(VOC) emissions are relevant due to known VOC
decay curves of the product. D Recycling potential:
Calculated benefits result from materials exclusive
B2 Maintenance: secondary materials (net materials).
Cleaning of the textile floor covering for a period of 1 D-A5: Benefits for generated energy due
year: to incineration of packaging and installation waste
Vacuum cleaning – electricity supply (incineration plant with R1 > 0.6),
Wet cleaning – electricity, water consumption, D-1: Benefits for generated energy due to landfill
production of the cleaning agent, waste water disposal of carpet waste at the end-of-life,
treatment D-2: Benefits for generated energy due to incineration
The declared values in this module have to be of carpet waste at the end-of-life (incineration plant
multiplied by the assumed service life of the floor with R1 > 0.6),
covering in the building in question. D-3: Benefits for saved fossil energy and saved
inorganic material due to recovery of the carpet in a
B3 - B5: cement plant.
The modules are not relevant within the assumed
reference service life of 10 years. Comparability
Basically, a comparison or an evaluation of EPD data
B6 - B7: is only possible if all the data sets to be compared
No energy and water input are required for the were created according to EN 15804 and the building
operation of the carpet in the use stage. The modules context, respectively the product-specific
do not cause any environmental impact. characteristics of performance, are taken into account.
C1 De-construction: Background data are taken from the GaBi database,
The floor covering is de-constructed manually and no 2022-2. Remaining data gaps are covered by the
additional environmental impact is caused. ecoinvent 3.7 database, 2020.
LCA: Scenarios and additional technical information
Characteristic product properties Transport to the construction site (A4)
Information on biogenic Carbon Name Value Unit
Litres of fuel (truck, EURO 0-6
0.012 l/100km
mix)
Name Value Unit Transport distance 700 km
Biogenic carbon content in Capacity utilisation (including
0 kg C 55 %
product at factory gate empty runs)
Biogenic carbon content in
accompanying packaging at 0.06 kg C Installation in the building (A5)
factory gate Name Value Unit
1 kg biogenic Carbon is equivalent to 44/12 kg of CO . Material loss 0.158 kg
2
Polyethylene packaging waste and installation waste
are considered to be incinerated in a municipal waste
incineration plant. Cardboard packaging waste is going
to be recycled.
Preparation of the floor and auxiliaries (adhesives,
fixing agents, PET connectors etc.) are not taken into
account.
4 Environmental Product Declaration modulyss – Tufted tiles, polyamide 6 with a maximum total pile weight of 1300 g/m2,
back2back or comfortback
Maintenance (B2) Reuse, recovery and/or recycling potentials (D),
The values for cleaning refer to 1 m2 floor covering per relevant scenario information
year. Recovery or recycling potentials due to the three end-
Depending on the application based on ISO 10874, the of-life scenarios (module C) are indicated separately.
technical service life recommended by the
manufacturer and the anticipated strain on the floor by Recycling in the cement industry (scenario 3)
customers, the case-specific useful life can be The organic material of the carpet is used as an
established. Based on this useful life the effects of alternative fuel in a cement kiln. It mainly substitutes
module B2 need to be calculated in order to obtain the for lignite (68.8%), hard coal (23.6%) and petrol coke
overall environmental impacts. (7.6%). The inorganic material is substantially
integrated into the cement clinker and substitutes for
original material input. VDZ e.V.
Name Value Unit
Maintenance cycle (vacuum Number
208
cleaning) /year
Number
Maintenance cycle (wet cleaning) 1,5
/year
Water consumption (wet cleaning) 0.004 m3
Cleaning agent (wet cleaning) 0.09 kg
Electricity consumption 0.314 kWh
For further information on cleaning and maintenance
see www.modulyss.com
Service life
Name Value Unit
Life Span (according to BBSR) 10 a
Corresponds to
Declared product properties (at the
-
the gate) and finishes specifications of
EN 1307
An assumed quality of work, when Conforms to the
installed in accordance with the manufacturer's -
manufacturer’s instructions instructions
Use in areas
defined by the
Usage conditions, e.g. frequency
use class -
of use, mechanical exposure
according to EN
1307
Maintenance e.g. required According to the
frequency, type and quality and manufacturers -
replacement of components instructions
End of Life (C1-C4)
Three different end-of-life scenarios are declared and
the results are indicated separately in module C.
Each scenario is calculated as a 100% scenario.
Scenario 1: 100 % landfill disposal
Scenario 2: 100 % municipal waste incineration (MWI)
with R1 > 0.6
Scenario 3: 100 % recovery in the cement industry
If combinations of these scenarios have to be
calculated this should be done according to the
following scheme:
EOL-impact = x % impact (Scenario 1)
+ y % impact (Scenario 2)
+ z % impact (Scenario 3)
with x % + y % + z % = 100 %
Name Value Unit
Collected as mixed construction
5.277 kg
waste (scenarios 1 and 2)
Collected separately (scenario 3) 5.277 kg
Landfilling (scenario 1) 5.277 kg
Energy recovery (scenario 2) 5.277 kg
Energy recovery (scenario 3) 2,822 kg
Recycling (scenario 3) 2.455 kg
5 Environmental Product Declaration modulyss – Tufted tiles, polyamide 6 with a maximum total pile weight of 1300 g/m2,
back2back or comfortback
LCA: Results
The LCA results refer to all declared products with a maximum total pile weight of 1300 g/m2. LCA results for
products with a maximum total pile weight of 480 g/m2 can be taken from the corresponding tables of the annexe.
Results for specific products with any other total pile weight can be calculated by using equation 1 given in the
annexe (see annexe chapter: 'General Information on the annexe'). The declared result figures in module B2 have
to be multiplied by the assumed service life (in years) of the floor covering in the building under consideration.
Information on non-relevant modules: Modules B3 - B7 are not relevant during the service life of the carpet.
Modules C1, C3/1, C4/2 and C4/3 cause no additional impact (see chapter "LCA: Calculation rules" in this
document). All these modules are declared and marked as 'modules not relevant/declared'. Module C2 represents
the transport for scenarios 1, 2 and 3. Column D represents module D/A5.
DESCRIPTION OF THE SYSTEM BOUNDARY (X = INCLUDED IN LCA; ND = MODULE OR INDICATOR NOT
DECLARED; MNR = MODULE NOT RELEVANT)
BENEFITS AND
CONSTRUCTI LOADS
PRODUCT STAGE ON PROCESS USE STAGE END OF LIFE STAGE BEYOND THE
STAGE SYSTEM
BOUNDARIES
6 Environmental Product Declaration modulyss – Tufted tiles, polyamide 6 with a maximum total pile weight of 1300 g/m2,
back2back or comfortback
lairetam
waR
ylppus tropsnarT
gnirutcafunaM
eht
morf
tropsnarT
etis
eht
ot
etag
ylbmessA esU
ecnanetniaM
riapeR
tnemecalpeR tnemhsibrufeR
ygrene
lanoitarepO esu
retaw
lanoitarepO esu
noitcurtsnoc-eD
noitilomed tropsnarT
gnissecorp
etsaW
lasopsiD -esueR -yrevoceR -gnilcyceR laitnetop
A1 A2 A3 A4 A5 B1 B2 B3 B4 B5 B6 B7 C1 C2 C3 C4 D
X X X X X X X MNR MNR MNR ND ND X X X X X
RESULTS OF THE LCA - ENVIRONMENTAL IMPACT according to EN 15804+A2: 1 m² floor covering
Core Indicator Unit A1-A3 A4 A5 B1 B2 C1 C2 C3/2 C3/3 C4/1 D D/1 D/2 D/3
-
GWP-total [kg CO2-Eq.] 1.51E+13.21E-1 8.89E-10.00E+04.16E-10.00E+01.79E-26.58E+06.65E+03.70E-1-6.07E-20.00E+0 1.78E+0-4.93E-1
-
GWP-fossil [kg CO2-Eq.] 1.53E+13.16E-1 6.81E-10.00E+02.15E-10.00E+01.76E-26.58E+06.65E+03.74E-1-6.04E-20.00E+0 1.77E+0-4.92E-1
GWP-biogenic [kg CO2-Eq.] -1.14E-14.09E-3 2.08E-10.00E+04.16E-30.00E+02.28E-4 8.58E-4 1.67E-30.00E+0-3.08E-40.00E+0-9.02E-3-7.15E-4
GWP-luluc [kg CO2-Eq.] 5.93E-3 1.79E-3 2.43E-40.00E+01.96E-10.00E+09.96E-5 2.60E-4 5.15E-4 1.82E-4-6.63E-60.00E+0-1.94E-4-2.24E-4
1.92E- 4.43E- 1.07E- 5.80E- 9.79E- 5.02E- -4.07E- -1.19E- -7.50E-
ODP [kg CFC11-Eq.] 1.48E-9 0.00E+03.42E-80.00E+0 0.00E+0
14 11 15 13 13 13 13 11 13
AP [mol H+-Eq.] 2.69E-2 1.91E-3 1.07E-30.00E+08.32E-40.00E+01.06E-4 6.49E-3 6.82E-3 1.11E-3-7.93E-50.00E+0-2.32E-3-1.69E-3
EP-freshwater [kg P-Eq.] 5.82E-5 9.57E-7 1.81E-60.00E+05.19E-60.00E+05.33E-8 9.55E-7 1.17E-6 6.98E-5-8.29E-80.00E+0-2.42E-6-5.10E-7
EP-marine [kg N-Eq.] 7.99E-3 9.37E-4 3.66E-40.00E+01.97E-40.00E+05.22E-5 3.18E-3 3.32E-3 2.45E-4-2.15E-50.00E+0-6.30E-4-5.31E-4
EP-terrestrial [mol N-Eq.] 7.08E-2 1.04E-2 3.53E-30.00E+02.83E-30.00E+05.78E-4 3.54E-2 3.70E-2 2.69E-3-2.31E-40.00E+0-6.75E-3-5.82E-3
POCP [kg NMVOC-Eq.]2.38E-2 1.77E-3 1.02E-3 4.18E-4 9.83E-40.00E+09.87E-5 8.15E-3 8.43E-3 7.89E-4-6.03E-50.00E+0-1.76E-3-1.61E-3
ADPE [kg Sb-Eq.] 2.28E-6 2.68E-8 7.03E-80.00E+02.30E-70.00E+01.49E-9 3.17E-8 4.28E-8 2.59E-8-9.10E-90.00E+0-2.66E-7-4.58E-8
- - -
ADPF [MJ] 3.18E+24.28E+09.80E+00.00E+05.90E+00.00E+02.39E-13.77E+04.86E+05.31E+0 0.00E+0
1.03E+0 3.00E+16.70E+1
[m³ world-Eq
WDP 1.79E+02.87E-3 8.12E-20.00E+09.99E-20.00E+01.60E-4 8.66E-1 8.73E-1-3.97E-3-6.35E-30.00E+0-1.86E-1-7.52E-2
deprived]
GWP = Global warming potential; ODP = Depletion potential of the stratospheric ozone layer; AP = Acidification potential of land and water; EP =
Caption Eutrophication potential; POCP = Formation potential of tropospheric ozone photochemical oxidants; ADPE = Abiotic depletion potential for non-
fossil resources; ADPF = Abiotic depletion potential for fossil resources; WDP = Water (user) deprivation potential
RESULTS OF THE LCA - INDICATORS TO DESCRIBE RESOURCE USE according to EN 15804+A2: 1 m²
floor covering
Indicator Unit A1-A3 A4 A5 B1 B2 C1 C2 C3/2 C3/3 C4/1 D D/1 D/2 D/3
PERE [MJ] 3.14E+1 2.44E-1 1.23E+0 0.00E+0 3.69E+0 0.00E+0 1.36E-2 6.30E-1 9.36E-1 4.36E-1 -2.81E-1 0.00E+0 -8.23E+0-6.36E-1
PERM [MJ] 2.54E-1 0.00E+0 -2.54E-1 0.00E+0 0.00E+0 0.00E+0 0.00E+0 0.00E+0 0.00E+0 0.00E+0 0.00E+0 0.00E+0 0.00E+0 0.00E+0
PERT [MJ] 3.17E+1 2.44E-1 9.77E-1 0.00E+0 3.69E+0 0.00E+0 1.36E-2 6.30E-1 9.36E-1 4.36E-1 -2.81E-1 0.00E+0 -8.23E+0-6.36E-1
PENRE [MJ] 2.44E+2 4.29E+0 1.00E+1 0.00E+0 5.90E+0 0.00E+0 2.39E-1 7.83E+1 7.94E+1 5.31E+0 -1.03E+0 0.00E+0 -3.00E+1-6.70E+1
PENRM [MJ] 7.48E+1 0.00E+0 -2.15E-1 0.00E+0 0.00E+0 0.00E+0 0.00E+0 -7.45E+1-7.45E+1 0.00E+0 0.00E+0 0.00E+0 0.00E+0 0.00E+0
PENRT [MJ] 3.18E+2 4.29E+0 9.81E+0 0.00E+0 5.90E+0 0.00E+0 2.39E-1 3.77E+0 4.86E+0 5.31E+0 -1.03E+0 0.00E+0 -3.00E+1-6.70E+1
SM [kg] 2.75E+0 0.00E+0 8.24E-2 0.00E+0 0.00E+0 0.00E+0 0.00E+0 0.00E+0 0.00E+0 0.00E+0 0.00E+0 0.00E+0 0.00E+0 1.90E-1
RSF [MJ] 0.00E+0 0.00E+0 0.00E+0 0.00E+0 0.00E+0 0.00E+0 0.00E+0 0.00E+0 0.00E+0 0.00E+0 0.00E+0 0.00E+0 0.00E+0 0.00E+0
NRSF [MJ] 0.00E+0 0.00E+0 0.00E+0 0.00E+0 0.00E+0 0.00E+0 0.00E+0 0.00E+0 0.00E+0 0.00E+0 0.00E+0 0.00E+0 0.00E+0 0.00E+0
FW [m³] 7.18E-2 2.75E-4 2.81E-3 0.00E+0 3.34E-3 0.00E+0 1.53E-5 2.05E-2 2.08E-2 6.22E-5 -2.69E-4 0.00E+0 -7.86E-3 -6.04E-3
PERE = Use of renewable primary energy excluding renewable primary energy resources used as raw materials; PERM = Use of
renewable primary energy resources used as raw materials; PERT = Total use of renewable primary energy resources; PENRE = Use of
non-renewable primary energy excluding non-renewable primary energy resources used as raw materials; PENRM = Use of non-
Caption
renewable primary energy resources used as raw materials; PENRT = Total use of non-renewable primary energy resources; SM = Use
of secondary material; RSF = Use of renewable secondary fuels; NRSF = Use of non-renewable secondary fuels; FW = Use of net fresh
water
RESULTS OF THE LCA – WASTE CATEGORIES AND OUTPUT FLOWS according to EN 15804+A2:
1 m² floor covering
Indicator Unit A1-A3 A4 A5 B1 B2 C1 C2 C3/2 C3/3 C4/1 D D/1 D/2 D/3
HWD [kg] 1.29E-3 2.06E-11 3.87E-5 0.00E+0 4.19E-5 0.00E+0 1.15E-125.65E-106.10E-108.19E-10-1.39E-100.00E+0 -4.07E-9-2.86E-10
NHWD [kg] 3.32E-1 6.15E-4 4.88E-2 0.00E+0 7.30E-3 0.00E+0 3.43E-5 1.29E+0 1.29E+0 5.26E+0 -5.18E-4 0.00E+0 -1.52E-2 -1.34E-1
RWD [kg] 6.00E-3 5.29E-6 1.84E-4 0.00E+0 3.76E-4 0.00E+0 2.95E-7 1.36E-4 2.15E-4 6.52E-5 -8.07E-5 0.00E+0 -2.36E-3 -1.35E-4
CRU [kg] 0.00E+0 0.00E+0 0.00E+0 0.00E+0 0.00E+0 0.00E+0 0.00E+0 0.00E+0 0.00E+0 0.00E+0 0.00E+0 0.00E+0 0.00E+0 0.00E+0
MFR [kg] 3.50E-2 0.00E+0 1.31E-1 0.00E+0 0.00E+0 0.00E+0 0.00E+0 0.00E+0 1.41E+0 0.00E+0 0.00E+0 0.00E+0 0.00E+0 0.00E+0
MER [kg] 0.00E+0 0.00E+0 0.00E+0 0.00E+0 0.00E+0 0.00E+0 0.00E+0 0.00E+0 0.00E+0 0.00E+0 0.00E+0 0.00E+0 0.00E+0 0.00E+0
EEE [MJ] 0.00E+0 0.00E+0 2.92E-1 0.00E+0 0.00E+0 0.00E+0 0.00E+0 8.62E+0 0.00E+0 0.00E+0 0.00E+0 0.00E+0 0.00E+0 0.00E+0
EET [MJ] 0.00E+0 0.00E+0 5.39E-1 0.00E+0 0.00E+0 0.00E+0 0.00E+0 1.60E+1 8.61E+1 0.00E+0 0.00E+0 0.00E+0 0.00E+0 0.00E+0
HWD = Hazardous waste disposed; NHWD = Non-hazardous waste disposed; RWD = Radioactive waste disposed; CRU = Components
Caption for re-use; MFR = Materials for recycling; MER = Materials for energy recovery; EEE = Exported electrical energy; EET = Exported
thermal energy
RESULTS OF THE LCA – additional impact categories according to EN 15804+A2-optional:
1 m² floor covering
Indicator Unit A1-A3 A4 A5 B1 B2 C1 C2 C3/2 C3/3 C4/1 D D/1 D/2 D/3
[Disease -6.57E-
PM 1.89E-7 1.10E-8 6.88E-9 0.00E+0 6.84E-8 0.00E+06.14E-10 2.83E-8 3.03E-8 1.07E-8 0.00E+0 0.00E+0 -2.29E-8
Incidence] 10
[kBq U235-
IRP 9.73E-1 7.75E-4 2.99E-2 0.00E+0 6.78E-2 0.00E+0 4.32E-5 2.08E-2 3.42E-2 9.63E-3 -1.37E-2 0.00E+0 0.00E+0 -1.45E-2
Eq.]
ETP-fw [CTUe] 1.58E+2 2.97E+0 4.89E+0 3.60E-3 2.69E+0 0.00E+0 1.66E-1 1.85E+0 2.48E+0 5.19E+0 -2.25E-1 0.00E+0 0.00E+0-1.17E+1
-1.04E- -1.27E-
HTP-c [CTUh] 4.68E-9 6.01E-111.45E-100.00E+06.21E-100.00E+03.35E-129.29E-111.07E-102.33E-10 0.00E+0 0.00E+0
11 10
-3.98E-
HTP-nc [CTUh] 2.01E-7 3.57E-9 6.34E-9 2.60E-11 9.46E-9 0.00E+01.99E-10 6.40E-9 7.12E-9 1.95E-8 0.00E+0 0.00E+0 -7.28E-9
10
SQP [-] ND ND ND ND ND 0.00E+0 ND ND ND ND ND ND ND ND
PM = Potential incidence of disease due to PM emissions; IR = Potential Human exposure efficiency relative to U235; ETP-fw = Potential
Caption comparative Toxic Unit for ecosystems; HTP-c = Potential comparative Toxic Unit for humans (cancerogenic); HTP-nc = Potential
comparative Toxic Unit for humans (not cancerogenic); SQP = Potential soil quality index
No substantiated values can be given for the SQP indicator with the existing database.
The result figures given in module B2 refer to a period of 1 year because a reference service life is not declared.
They have to be multiplied by the assumed service life (in years) of the floor covering in the building under
consideration.
Disclaimer 1 – for the indicator “Potential Human exposure efficiency relative to U235”.
This impact category deals mainly with the eventual impact of low-dose ionizing radiation on human health of the
nuclear fuel cycle. It does not consider effects due to possible nuclear accidents, occupational exposure or
radioactive waste disposal in underground facilities. Potential ionizing radiation from the soil, from radon and from
some construction materials is also not measured by this indicator.
Disclaimer 2 – for the indicators “abiotic depletion potential for non-fossil resources”, “abiotic depletion potential
for fossil resources”, “water (user) deprivation potential, deprivation-weighted water consumption”, “potential
comparative toxic unit for ecosystems”, “potential comparative toxic unit for humans – cancerogenic”, “Potential
comparative toxic unit for humans - not cancerogenic”, “potential soil quality index”.
The results of this environmental impact indicator shall be used with care as the uncertainties on these results are
high or as there is limited experience with the indicator.
References
EN 1307 floor coverings – Environmental product declarations –
DIN EN 1307: 2014+A1:2016+A2:2018-05: Textile Product category rules
floor coverings - Classification
ISO 10874
EN 13501-1 DIN EN ISO 10874: 2012+A1:2021-04: Resilient,
DIN EN 13501-1:2019-05: Fire classification of textile and laminate floor coverings - Classification
construction products and building elements - Part 1:
Classification using data from reaction to fire tests ISO 14025
DIN EN /ISO 14025:2011-10/, Environmental labels
EN 14041 and declarations — Type III environmental
DIN EN 14041: 2018-05 and DIN EN 14041: 2008-05: declarations — Principles and procedures
Resilient, textile and laminate floor coverings -
Essential characteristics
ISO 14040
EN 15804 DIN EN ISO 14040:2006+A1:2020 Environmental
DIN EN 15804:2012+A2:2019+AC:2021, Sustainability management - Life cycle assessment - Principles and
of construction works — Environmental Product framework
Declarations — Core rules for the product category of
construction products ISO 14044
DIN EN ISO 14044:2006+A1:2018+A2:2020
EN 16810 Environmental management - Life cycle assessment -
DIN EN 16810: 2017-08: Resilient, textile and laminate Requirements and guidelines
7 Environmental Product Declaration modulyss – Tufted tiles, polyamide 6 with a maximum total pile weight of 1300 g/m2,
back2back or comfortback
ISO 15686 GaBi database
ISO 15686: Buildings and constructed assets - GaBi Software-System and Database for Life Cycle
Service life planning Engineering, thinkstep AG, Leinfelden-Echterdingen,
ISO 15686-1: 2011-05: Part 1: General principles and 2022-2
framework
ISO 15686-2: 2012-05: Part 2: Service life prediction PCR Part A
procedures Product Category Rules for Building-Related Products
ISO 15686-7: 2017-04: Part 7: Performance and Services Part A: Calculation Rules for the Life
evaluation for feedback of service life data Cycle Assessment and Requirements on the Project
from practice Report according to EN 15804+A2:2019, V1.1, Berlin:
ISO 15686-8: 2008-06: Part 8: Reference service life Institut Bauen und Umwelt e.V. (IBU), January 2021
and service-life estimation
PCR Part B
Regulation (EU) No. 305/2011 Product Category Rules for Building-Related Products
Regulation No. 305/2011 Construction Products and Services
Regulation (CPR) of the European Council and of the Part B: Requirements on the EPD for floor coverings,
European Parliament, April 2011 V1.2, Berlin: Institut Bauen und Umwelt e.V. (IBU),
February 2018
General Instructions for the IBU-EPD Program
General Instructions for the EPD-Program of the PRODIS
Institut Bauen und Umwelt e.V., The Preparation of Product Information System (PRODIS) of the
Environmental Product Declarations - EPDs, version European Carpet Industry, Gemeinschaft
2.0, Institut Bauen und Umwelt e.V., Berlin, January umweltfreundlicher Teppichboden e.V (GUT) and
2021, www.ibu-epd.de European Carpet and Rug Association
(ECRA), http://www.pro-dis.info
BNB, Nutzungsdauer von Bauteilen
Bewertungssystem Nachhaltiges Bauen (BNB), REACH
Nutzungsdauer von Bauteilen, Bundesministerium des Regulation (EC) No 1907/2006 of the European
Inneren, für Bau und Heimat, 24.02.2017 Parliament and of the Council of 18 December 2006
concerning the Registration, Evaluation, Authorisation
ECHA candidate list and Restriction of Chemicals (REACH), June 2017,
Candidate List of substances of very high concern last update: 08.07.2021
(SVHCs) for authorisation, 08.07.2021, European
Chemicals Agency (ECHA), Helsinki, Finland VDZ e.V.
Association of German Cement Works, Ed. Environ-
mental Data of the German Cement Industry 2020
ecoinvent
ecoinvent, Zurich, Switzerland, database version 3.7,
published September 2020
8 Environmental Product Declaration modulyss – Tufted tiles, polyamide 6 with a maximum total pile weight of 1300 g/m2,
back2back or comfortback
Publisher
Institut Bauen und Umwelt e.V. Tel +49 (0)30 3087748- 0
Hegelplatz 1 Fax +49 (0)30 3087748- 29
10117 Berlin Mail info@ibu-epd.com
Germany Web www.ibu-epd.com
Programme holder
Institut Bauen und Umwelt e.V. Tel +49 (0)30 - 3087748- 0
Hegelplatz 1 Fax +49 (0)30 – 3087748 - 29
10117 Berlin Mail info@ibu-epd.com
Germany Web www.ibu-epd.com
Author of the Life Cycle
Assessment Tel +49 (0)241 96843 410
Gemeinschaft umweltfreundlicher Fax +49 (0)241 96843 400
Teppichboden (GUT) e.V. Mail mail@gut-ev.de
Schönebergstraße 2 Web www.gut-ev.org
52068 Aachen
Germany
Owner of the Declaration
modulyss Tel +32 (0)52 45 72 11
Zevensterrestraat 21 Fax +32 (0)52 44 90 99
9240 Zele Mail info@modulyss.com
Belgium Web www.modulyss.com
