ENVIRONMENTAL PRODUCT DECLARATION
as per ISO 14025 and EN 15804+A2
Owner of the Declaration NedZink B.V.
Programme holder Institut Bauen und Umwelt e.V. (IBU)
Publisher Institut Bauen und Umwelt e.V. (IBU)
Declaration number EPD-NED-20200257-IBA1-EN
Issue date 22.03.2022
Valid to 21.03.2027
NedZink NOVA, NedZink NEO, NedZink NOIR
NedZink B.V.
www.ibu-epd.com | https://epd-online.com
Umwelt Produktdeklaration Name des Herstellers – Name des Produkts
1. General Information
NedZink B.V. NedZink® NOVA / NedZink® NEO /
NedZink® NOIR
Programme holder Owner of the declaration
IBU – Institut Bauen und Umwelt e.V. NedZink B.V.
Panoramastr. 1 Hoofdstraat 1
10178 Berlin 6024 AA, Budel-Dorplein
Germany Netherlands
Declaration number Declared product / declared unit
EPD-NED-20200257-IBA1-EN 1kg NedZink® NOVA/NedZink® NEO/NedZink® NOIR,
pre-weathered titanium zinc
This declaration is based on the product Scope:
category rules: The Life Cycle Assessment (LCA) was carried out
Building metals, 11.2017 according to ISO 14040, ISO 14044 and EN 15804.
(PCR checked and approved by the SVR) The LCA is performed for the pre-weathered products
NedZink® NOVA/NedZink® NEO/NedZink® NOIR
manufactured by NedZink B.V. in Budel-Dorplein,
Issue date
Netherlands.
22.03.2022
The pre-weathered rolled zinc from NedZink covered
by this EPD can be used in buildings as roof, façade or
Valid to rainwater systems. The LCA was carried out for the
21.03.2027 manufacturing phase of the declared product,
containing information on raw and secondary material
production, transport and packaging (cradle to gate).
Possible credits after the end of life phase (module D),
demolition (C1), transport to waste processing and
disposal (C2), waste processing (C3) and waste
disposal (C4) are also included.
The owner of the declaration shall be liable for the
underlying information and evidence; the IBU shall not
be liable with respect to manufacturer information, life
cycle assessment data and evidences.
The EPD was created according to the specifications
of EN 15804+A2. In the following, the standard will be
simplified as EN 15804.
Verification
The standard EN 15804 serves as the core PCR
Independent verification of the declaration and data
according to ISO 14025:2010
Dipl. Ing. Hans Peters internally x externally
(chairman of Institut Bauen und Umwelt e.V.)
Dr. Alexander Röder Mr Olivier Muller
(Managing Director Institut Bauen und Umwelt e.V.)) (Independent verifier)
2. Product
2.1 Product description/Product definition Product certificate (approval No QIS 122). The defined
NedZink® NOVA/NedZink® NEO/NedZink® NOIR is material properties are checked by an independent
pre-weathered titanium zinc produced by NedZink and neutral research institute.
according to EN 988. This product certification and the ISO 9001 certificate
Small quantities, as specified in EN 988, of the alloy for the quality management system at NedZink assure
elements copper, titanium and aluminium are added to a constant and uniform high-quality standard.
electrolytically refined zinc (with a purity of min.
99,995% Zn, Z1 according to EN 1179). NedZink® NOVA is pre-weathered titanium zinc in a
The chemical composition, mechanical and physical matt natural medium grey colour. NedZink® NEO is
properties and measurement tolerances are pre-weathered titanium zinc in a matt natural mineral
determined in the KOMO product certificate and grey colour. NedZink® NOIR is pre-weathered titanium
certified as NedZink NTZ® by Lloyd's Register zinc in an anthracite black colour.
2 Environmental Product Declaration NedZink B.V. – NedZink NOVA, NedZink NEO, NedZink NOIR
For the placing on the market of the product in the 2.5 Base materials/Ancillary materials
European Union/European Free Trade Association Components of NedZink alloy
(EU/EFTA) (with the exception of Switzerland) The composition of pre-weathered rolled zinc from
Regulation (EU) No. 305/2011 (CPR) applies. The NedZink is in accordance with EN988:
product needs a Declaration of Performance taking - Special-High-Grade zinc 99.995% (Z1 according to
into consideration EN 14782:2006, Self-supporting EN 1179)
metal sheet for roofing, external cladding and internal - Copper: 0.08 - 0.17%
lining, or EN 14783:2013, Fully supported metal sheet - Titanium: 0.07 - 0.12%
and strip for roofing, external cladding and internal - Aluminium: ≤ 0.015%
lining, and the CE-marking.
For the application and use the respective national Auxiliary substances
provisions apply. Lubricant oil: 0.89 kg/t zinc; a number of different
agents for cleaning, activating and phosphating;
2.2 Application temporary protection: 1 - 1.5 µm thickness
NedZink® NOVA/NedZink® NEO/NedZink® NOIR
titanium zinc coils, sheets, strips and profiles are used None of the components included in the final product is
for: listed in the Candidate List of Substances of Very High
- roof and façade cladding (CE-marked based Concern for Authorisation (SVHC) dated 01/2018.
on EN14782:2006, Self-supporting metal sheet The product does not contain substances
for roofing, external cladding and internal lining with carcinogenic mutagenic reprotoxic (CMR)
or EN14783:2013, Fully supported metal sheet and properties >0.1%.
strip for roofing, external cladding and internal lining)
- interior use This product/article/at least one partial article contains
- roof drainage systems (gutters, downpipes and substances listed in the candidate list (dated 01/2018)
accessories according to EN612) exceeding 0.1 percentage by mass: no
- ornaments
This product/article/at least one partial article contains
2.3 Technical Data other CMR substances in categories 1A or 1B which
The main constructional data are presented in the are not on the candidate list, exceeding 0.1 percentage
following table: by mass: no
Constructional data Biocide products were added to this construction
Name Value Unit product or it has been treated with biocide products
Coefficient of thermal expansion 22 10-6K-1 (this then concerns a treated product as defined by the
Tensile strength ≥ 150 N/mm2 (EU) Ordinance on Biocide Products No.
not 528/2012): no
Compressive strength N/mm2
relevant
Modulus of elasticity ≥ 80000 N/mm2
Melting point 420 °C 2.6 Manufacture
Thermal conductivity 110 W/(mK) The manufacturing process of pre-weathered rolled
Electrical conductivity at 20°C 17000000 Ω-1m-1 zinc includes the following steps:
Density 7200 kg/m3
Pre-alloy:
Required testing standards are described in EN 988.
In order to improve the properties of zinc, and for
energy saving purposes, a pre-alloy with titanium,
Performance data of the product in accordance with
copper and aluminium is prepared in an induction
the declaration of performance with respect to its
furnace. This pre-alloy is poured into ingots.
essential characteristics according to EN
14782 and EN 14783 respectively.
Melting:
In the melting furnace the Special High Grade (SHG)
2.4 Delivery status
zinc and the ingots are mixed homogeneously. Zinc
NedZink material is delivered in thicknesses from 0.5
with the right composition is pumped to the casting
to 1.5 mm. As average production data is considered,
furnace.
the LCIA results reflect the environmental profile of
weighted average product thickness: 0.750 mm.
Casting:
The maximum width of sheets, coils and strips is 1000
Casting takes place from the casting furnace into a
mm.
vertical casting installation. The zinc is cast into blocks,
The standard sheets are delivered in 1000 x 2000 mm,
cooled down with a closed water system and stored for
1000 x 2250 mm and 1000 x 3000 mm.
further processing.
Finished products are delivered to customer
specification.
Rolling and coiling:
Blocks coming from the casting installation are
Application rules:
homogeneous pre-heated for the “hot rolling” process.
EN988:1996, Zinc and zinc alloys - Specifications for
This takes place in a gas-fired continuous oven.
rolled flat products for buildings
During the hot rolling on a reversible rolling machine
EN612:2005, Eaves gutters with bead stiffened fronts
the blocks are processed to a predefined thickness. At
and rainwater pipes with seamed joints made of metal
the end of the rolling installation the zinc is coiled and
sheet
stored to cool off.
On the reversible cold-rolling mill the coils are rolled to
the desired final thickness. For cooling and lubrication
of the process a special emulsion is used
3 Environmental Product Declaration NedZink B.V. – NedZink NOVA, NedZink NEO, NedZink NOIR
2.9 Packaging
Stretching and cutting: The packaging material in use are wooden pallets,
Tension in the coils is released by a stretching- and paper/cardboard and plastics (films and wires). All
straightening process. The zinc is uniquely marked and packaging materials are reusable and/or recyclable, if
slitted and cut to the desired width and length. gathered separately.
The take-back and recycling of our packaging in
Pre-weathering: Germany is organized by Interseroh.
In a continuously operating production line the coils are
degreased, brushed and phosphated to get a
prepatinated medium grey appearance for NedZink® 2.10 Condition of use
NOVA or a mineral grey appearance for NedZink® NedZink material develops a protective patina layer,
NEO. which darkens the material slightly over time due to a
With an additional process for NedZink® NOIR an reaction with oxygen and carbon dioxide (air and
anthracite black appearance is created. After rinsing water).
and drying the material surface is provided with a thin This layer is responsible for the high resistance of
transparent protection layer and stored in the titanium zinc against corrosion. For both pre-
warehouse. weathered zinc and natural rolled zinc this behaviour is
the same.
Quality control: Zinc in contact with air creates a zinc-oxide. Due to the
During the entire process extensive quality checks are influence of water, a zinc-hydroxide is developed. In
conducted by the manufacturer and Lloyd's Register. the final step, a reaction with carbon dioxide creates a
Quality Management according to ISO 9001. non-water-soluble coating of basic zinc carbonate,
Product quality is checked by Lloyd's Register and being the patina.
approved with an Industrial Quality Scheme Approval Therefore NedZink material does not require any
Certificate QIS122. maintenance and cleaning during the period of use. If
the surface is slightly damaged, this naturally formed
Additionally, the quality control is audited by Kiwa and patina layer will heal itself.
certified with KOMO product certificates:
- BRL2034, KOMO K7054/04 zinc sheets NedZink material is UV-resistant, non-flammable and
- BRL2035, KOMO K7057/04 zinc gutters resistant to radiating heat. Direct contact with chemical
- BRL2044, KOMO K7063/04 zinc downpipes substances, especially those containing acids, has to
be avoided. A list of substances to be avoided can be
2.7 Environment and health during found on www.nedzink.com.
manufacturing
The manufacturing process is carried out according to The material has a repellent effect to electrosmog
the rules as laid down in the environmental permit. (electromagnetic radiation) and the effects of rain and
NedZink’s policy follows the Total Quality Management snow may be neglected.
(TQM).
The directives of the Environmental Management 2.11 Environment and health during use
System ISO14001 are an integral part of the Quality Environment
Management System ISO9001. The due to air and water formed patina (zinc
carbonate) is a natural protection layer. Due to this
2.8 Product processing/Installation patina the transfer of zinc ions via rain water is
Basic principles: constantly reduced, because this protection layer is
NedZink material must be stored under dry and non-water-soluble.
ventilated conditions. This applies to storage in Further transfer of zinc ions is mainly related to the air
warehouses, on building sites, on installation sites as pollution with SO . Due to the reduction of SO
2 2
well as during transportation. Coils are to be stored on concentration in the air, the zinc-concentration of
their original pallets. precipitation in the rainwater has subsequently been
reduced to one fifth of the former values during the last
Transportation should only be done in enclosed thirty years.
vehicles.
As a result of all environmental regulations this amount
Temperature deviations have to be avoided as it can will reduce even more in the future, due to the
result in varying humidity levels. reduction of SO concentration in the air. The transfer
2
All contact between zinc and moisture (wet surface, of zinc ions via rain water is constantly reduced due to
rain or dew) during handling and transportation must the development of a natural protection layer of zinc
be avoided. Wet surfaces (with or without protective carbonate.
film) may not directly be covered.
In aquatic systems only a small part of the total zinc
The material is to be processed without tension. concentration is available for organisms (bioavailable).
It is related to the physical-chemical conditions of the
The thermal expansion has to be taken into account receiving water body.
when installing/handling the product.
Health
Mechanical deformation of zinc should be avoided in When used according to their designated function,
case the zinc temperature is not at least 7°C. NedZink products will have no health effects.
Zinc is an essential metal, necessary for living
Further installation rules are listed on organisms. Zinc does not accumulate in the body.
www.nedzink.com. The recommended daily intake of zinc (in the correct
4 Environmental Product Declaration NedZink B.V. – NedZink NOVA, NedZink NEO, NedZink NOIR
form) according to the WHO is 15mg/day for men Water
and12mg/day for women. Zinc is not classified as hazardous for the aquatic
environment.
2.12 Reference service life
The service life depends on the correct application Mechanical destruction
according to the guidelines for processing and Given the metallic nature of the product, there will be
installation. The theoretical lifetime according to the no environmental effect.
available literature is > 100 years.
Service lifetime according to Bundesinstitut für Bau-, 2.14 Re-use phase
Stadt- und Raumforschung (BBSR): > 50 years. Disassembly:
During disassembly of a building construction or
As the EPD scope is a cradle-to-gate with options, no renovations, NedZink material should be separated
reference service life is declared in the LCA. from other materials. Zinc can then easily be collected
for re-use and/or recycling.
The standard ISO 15686 has not been considered.
Re-use/Recycling:
Scrap produced during the manufacturing process
2.13 Extraordinary effects from NedZink material are 100% remelted and fed
back completely into NedZink's production process. A
Fire small amount of residue (skimmings, dross, dust),
The NedZink® products comply with EN13501-1: the which is no longer valuable for the internal production
requirements of building material Class A1 "non- process, is completely recycled by a third party
combustible". (96/603/EC) (European Waste Code 10.05.01).
Fire protection The scrap from demolition and renovation work on
Name Value building sites is collected and sold either directly to
Building material class EN13501 secondary smelting works or via a scrap metal dealer.
A1
DIN4102 The recycling rate for zinc sheets is over 95%. Credits
Burning droplets EN13501 D0 for this recycling are appointed in module D. These
Smoke gas development credits are based on a recycling percentage of 95%
-
EN13501 (European recycling rate for rolled zinc).
Smoke production 2.15 Disposal
Vaporization as zinc oxide (ZnO) occurs when heated Due to the effective recycling process, a maximum of
above 650 °C. The produced ZnO smoke may cause 5% zinc has to be disposed.
zinc fever (diarrhoea, dry throat, feverish) when The European Waste Code for collected zinc after
inhaled over some (period of) time. The effects disassembly is 17.04.04.
disappear completely in 1 to 2 days after the
inhalation. 2.16 Further information
Additional information, optional details, references,
data sheets can be obtained at: www.nedzink.com
3. LCA: Calculation rules
3.1 Declared Unit
The declared unit is 1 kg of NedZink® NOVA/ 3.4 Cut-off criteria
NedZink® NEO/NedZink® NOIR, pre-weathered No major cut-offs were applied to specific
titanium zinc. manufacturing data from Nedzink. Production impacts
of packaging for raw materials are not known and
Declared unit excluded, waste processing of this packaging is known
Name Value Unit and included. For upstream data a background
Declared unit 1 kg database (Ecoinvent V3.6) was used, which can
conversion factor [Mass/Declared contain additional cut-offs.
1 -
Unit]
Gross density 7200 kg/m3 3.5 Background data
Background processes are taken from the Ecoinvent
V3.6 database (2019), with the “allocation, cut-off by
classification” system model.
3.2 System boundary Life cycle inventory data for the production of zinc
Type of the EPD: Cradle-to-Gate with options. Modules concentrate and SHG Zinc in the Ecoinvent V3.6
A1, A2 and A3 contain information on the raw- and database is updated with the most recent LCA report
secondary material extraction, transport to the (Zinc Environmental Profile - 2015 Update) on primary
manufacturer, manufacturing and packaging. Zinc by the International Zinc Association (IZA).
Module C1 - C4 (end of life) and module D (applicable The environmental impact of the SHG Zinc was then
to the aforementioned modules) are declared. Modules calculated using SimaPro V9.0. Site-specific data was
A4, A5 and B1-B7 are not declared. provided by NedZink and verified against earlier
studies.
3.3 Estimates and assumptions
No major estimates or assumptions were required for
the creation of this EPD.
5 Environmental Product Declaration NedZink B.V. – NedZink NOVA, NedZink NEO, NedZink NOIR
3.6 Data quality However, the following allocation had to be done:
The data used for this study was both of high quality - For pre-weathered zinc, there is a net output stream
and recent. The specific data was collected by the of rejected zinc product to internal recycling. As this is
manufacturer, The generic data that is used is less an internal recycling process, 0 impacts are allocated
than 10 years old or has been updated within this to this material flow.
period. This is in compliance with the data quality
requirements of EN 15804. 3.9 Comparability
Basically, a comparison or an evaluation of EPD data
3.7 Period under review is only possible if all the data sets to be compared
Site-specific data for the years 2019 and 2020 was were created according to EN 15804 and the building
used in this study. Background data is taken from the context, respectively the product-specific
Ecoinvent V3.6 database (2019) and varies in age. characteristics of performance, are taken into account.
3.8 Allocation The used background database is Ecoinvent
Allocation was avoided as much as possible in this V3.6 database (2019).
study, as required in EN 15804.
4. LCA: Scenarios and additional technical information
Characteristic product properties
Information on biogenic Carbon
The biogenic carbon content quantifies the amount of
biogenic carbon in a construction product leaving the
factory gate, and it shall be separately declared for the
product and for any accompanying packaging.
If the total mass of biogenic carbon containing
materials is less than 5 % of the total mass of the
product and accompanying packaging, the declaration
of biogenic carbon content may be omitted. The mass
of packaging containing biogenic carbon shall always
be declared.
Note: 1 kg biogenic Carbon is equivalent to 44/12 kg of
CO
2
Modules A4, A5, B1-B7 are not considered in this
study. The possible credits given in Module D are
based on 100% recyclability of zinc products. After the
collection (a collection rate of 95% is taken), zinc scrap
is re-melted and converted to secondary zinc. This is
not done by NedZink but by third parties. The possible
credit for the zinc gained through re-melting is
calculated using the dataset of the primary zinc
production. The remaining zinc (5%) is landfilled
(module C4).
End of life (C4) / Recycling potentials (D)
Name Value Unit
Recycling 95% kg
Landfilling 5% kg
6 Environmental Product Declaration NedZink B.V. – NedZink NOVA, NedZink NEO, NedZink NOIR
5. LCA: Results
Disclaimer:
EP-freshwater: This indicator has been calculated as “kg P eq” as required in the characterization model
(EUTREND model, Struijs et al., 2009b, as implemented in ReCiPe;
http://eplca.jrc.ec.europa.eu/LCDN/developerEF.xhtml)
DESCRIPTION OF THE SYSTEM BOUNDARY (X = INCLUDED IN LCA; ND = MODULE OR INDICATOR NOT
DECLARED; MNR = MODULE NOT RELEVANT)
BENEFITS AND
CONSTRUCTI LOADS
PRODUCT STAGE ON PROCESS USE STAGE END OF LIFE STAGE BEYOND THE
STAGE SYSTEM
BOUNDARIES
7 Environmental Product Declaration NedZink B.V. – NedZink NOVA, NedZink NEO, NedZink NOIR
lairetam
waR
ylppus tropsnarT
gnirutcafunaM
eht
morf
tropsnarT
etis
eht
ot
etag
ylbmessA esU
ecnanetniaM
riapeR
tnemecalpeR tnemhsibrufeR
ygrene
lanoitarepO esu
retaw
lanoitarepO esu
noitcurtsnoc-eD
noitilomed tropsnarT
gnissecorp
etsaW
lasopsiD -esueR -yrevoceR -gnilcyceR laitnetop
A1 A2 A3 A4 A5 B1 B2 B3 B4 B5 B6 B7 C1 C2 C3 C4 D
X X X ND ND ND ND MNR MNR MNR ND ND X X X X X
RESULTS OF THE LCA - ENVIRONMENTAL IMPACT according to EN 15804+A2: 1 kg NEDZINK
NOVA/NEO/NOIR
Core Indicator Unit A1-A3 C1 C2 C3 C4 D
Global warming potential - total [kg CO2-Eq.] 4.73E+0 1.73E-4 6.92E-3 5.73E-2 2.64E-4 -2.91E+0
Global warming potential - fossil fuels [kg CO2-Eq.] 4.56E+0 1.73E-4 6.91E-3 5.72E-2 2.63E-4 -2.78E+0
Global warming potential - biogenic [kg CO2-Eq.] 1.50E-1 4.82E-8 4.20E-6 3.09E-5 5.22E-7 -1.21E-1
GWP from land use and land use change [kg CO2-Eq.] 1.36E-2 1.37E-8 2.45E-6 9.83E-6 7.34E-8 -9.49E-3
Depletion potential of the stratospheric ozone layer [kg CFC11-Eq.] 3.72E-7 3.74E-11 1.59E-9 1.19E-8 1.08E-10 -2.08E-7
Acidification potential, accumulated exceedance [mol H+-Eq.] 4.39E-2 1.81E-6 3.94E-5 5.84E-4 2.50E-6 -2.75E-2
Eutrophication, fraction of nutrients reaching freshwater
end compartment
[kg PO4-Eq.] 4.58E-4 6.31E-10 5.69E-8 3.48E-7 2.95E-9 -3.26E-4
Eutrophication, fraction of nutrients reaching marine end
[kg N-Eq.] 8.54E-3 8.01E-7 1.41E-5 2.54E-4 8.60E-7 -5.94E-3
compartment
Eutrophication, accumulated exceedance [mol N-Eq.] 9.66E-2 8.78E-6 1.55E-4 2.79E-3 9.48E-6 -6.71E-2
Formation potential of tropospheric ozone photochemical
[kg NMVOC-Eq.] 2.48E-2 2.42E-6 4.44E-5 7.67E-4 2.75E-6 -1.67E-2
oxidants
Abiotic depletion potential for non-fossil resources [kg Sb-Eq.] 9.30E-2 2.66E-10 1.79E-7 9.37E-8 2.41E-9 -7.32E-2
Abiotic depletion potential for fossil resources [MJ] 6.69E+1 2.39E-3 1.06E-1 7.85E-1 7.36E-3 -4.14E+1
Water (user) deprivation potential, deprivation-weighted [m³ world-Eq
3.87E+0 3.20E-6 3.26E-4 1.43E-3 3.30E-4 -3.01E+0
water consumption (WDP) deprived]
RESULTS OF THE LCA - INDICATORS TO DESCRIBE RESOURCE USE according to EN 15804+A2: 1 kg
NEDZINK NOVA/NEO/NOIR
Indicator Unit A1-A3 C1 C2 C3 C4 D
Renewable primary energy as energy carrier [MJ] 8.73E+0 1.29E-5 1.52E-3 8.27E-3 5.95E-5 -5.62E+0
Renewable primary energy resources as material utilization [MJ] 2.01E-1 0.00E+0 0.00E+0 0.00E+0 0.00E+0 0.00E+0
Total use of renewable primary energy resources [MJ] 8.93E+0 1.29E-5 1.52E-3 8.27E-3 5.95E-5 -5.62E+0
Non-renewable primary energy as energy carrier [MJ] 7.14E+1 2.53E-3 1.13E-1 8.34E-1 7.82E-3 -4.40E+1
Non-renewable primary energy as material utilization [MJ] 0.00E+0 0.00E+0 0.00E+0 0.00E+0 0.00E+0 0.00E+0
Total use of non-renewable primary energy resources [MJ] 7.14E+1 2.53E-3 1.13E-1 8.34E-1 7.82E-3 -4.40E+1
Use of secondary material [kg] 0.00E+0 0.00E+0 0.00E+0 0.00E+0 0.00E+0 9.47E-1
Use of renewable secondary fuels [MJ] 0.00E+0 0.00E+0 0.00E+0 0.00E+0 0.00E+0 0.00E+0
Use of non-renewable secondary fuels [MJ] 0.00E+0 0.00E+0 0.00E+0 0.00E+0 0.00E+0 0.00E+0
Use of net fresh water [m³] 1.20E-1 1.23E-7 1.20E-5 5.87E-5 7.86E-6 -8.95E-2
RESULTS OF THE LCA – WASTE CATEGORIES AND OUTPUT FLOWS according to EN 15804+A2:
1 kg NEDZINK NOVA/NEO/NOIR
Indicator Unit A1-A3 C1 C2 C3 C4 D
Hazardous waste disposed [kg] 1.18E-2 6.50E-9 2.71E-7 2.06E-6 1.10E-8 -9.46E-3
Non-hazardous waste disposed [kg] 6.39E-1 2.83E-6 6.57E-3 1.06E-3 5.00E-2 -4.08E-1
Radioactive waste disposed [kg] 3.06E-4 1.66E-8 7.21E-7 5.32E-6 4.83E-8 -2.14E-4
Components for re-use [kg] 0.00E+0 0.00E+0 0.00E+0 0.00E+0 0.00E+0 0.00E+0
Materials for recycling [kg] 1.88E-1 1.19E+0 2.19E+0 3.19E+0 0.00E+0 0.00E+0
Materials for energy recovery [kg] 0.00E+0 0.00E+0 0.00E+0 0.00E+0 0.00E+0 0.00E+0
Exported electrical energy [MJ] 0.00E+0 0.00E+0 0.00E+0 0.00E+0 0.00E+0 0.00E+0
Exported thermal energy [MJ] 0.00E+0 0.00E+0 0.00E+0 0.00E+0 0.00E+0 0.00E+0
RESULTS OF THE LCA – additional impact categories according to EN 15804+A2-optional:
1 kg NEDZINK NOVA/NEO/NOIR
Indicator Unit A1-A3 C1 C2 C3 C4 D
Potential incidence of disease due to PM emissions [Disease
1.68E-7 4.80E-11 6.24E-10 1.52E-8 4.85E-11 -9.62E-8
Incidence]
Potential Human exposure efficiency relative to U235 [kBq U235-
4.17E-1 1.02E-5 4.64E-4 3.37E-3 3.02E-5 -3.08E-1
Eq.]
Potential comparative toxic unit for ecosystems [CTUe] 8.61E+2 1.44E-3 8.61E-2 5.04E-1 4.77E-3 -6.61E+2
Potential comparative toxic unit for humans - cancerogenic [CTUh] 2.12E-8 5.03E-14 3.07E-12 1.68E-11 1.10E-13 -1.62E-8
Potential comparative toxic unit for humans - not cancerogenic [CTUh] 6.28E-7 1.24E-12 1.03E-10 4.19E-10 3.41E-12 -4.80E-7
Potential soil quality index [-] 3.26E+1 3.05E-4 9.07E-2 1.16E-1 1.54E-2 -2.13E+1
Disclaimer 1 – for the indicator IRP:
This impact category deals mainly with the eventual impact of low dose ionizing radiation on human health of the
nuclear fuel cycle. It does not consider effects due to possible nuclear accidents, occupational exposure nor (due
to) radioactive waste disposal in underground facilities. Potential ionizing radiation from the soil, from radon and
(from) some construction materials is also not measured by this indicator.
Disclaimer 2 – for the indicators ADPE, ADPF, WDP, ETP-fw, HTP-c, HTP-nc, SQP:
The results of this environmental impact indicator shall be used with care as the uncertainties on these results are
high or as there is limited experience with the indicator.
6. LCA: Interpretation
The main impact categories for 1 kg of Nedzink Nova, The remaining contributions mainly consist of energy
Neo, Noir usage (electricity and gas), substances used for pre-
weathering and a small contribution from the remaining
Life cycle inventory data for the production of zinc metal components (Cu, Ti, Al).
concentrate and Special High-Grade Zinc (SHG Zinc)
in the background database Ecoinvent V3.6 is aligned Because of the high contribution of SHG Zinc and the
with data from the IZA 2015 LCA report (Zinc high recyclability that is assumed, the amount of
Environmental Profile - 2015 Update, see also section credits gained in module D for each impact category is
3.5 Background Data). high, at least 59% or higher compared to the initial
impact value.
The contribution of SHG Zinc is the dominating factor
in all of the impact categories, with contributions >70%
in for all indicators.
7. Requisite evidence
In a literature study TNO-MEP-99/441 of TNO (Dutch influenced by the atmospheric conditions, of which the
Organisation for Applied Scientific Research) the SO concentration is the most important variable. With
2
emissions from corrosion of zinc to water have been the decreasing of the SO concentration, the corrosion
2
evaluated. This corrosion rate refers to the loss of rate is also decreasing.
metallic zinc.
The run-off rate is the wash-off of zinc from the patina
layer. This run-off rate is generally lower than the In areas with higher SO -concentration a run-off rate of
2
corrosion rate. 3 g/m2.yr can be calculated and 2 g/m2.yr in areas with
lower concentration.
During the built-up of the zinc patina layer the run-off is
lower than the corrosion rate. The growth of the patina
layer delays the corrosion. The run-off rate is
8 Environmental Product Declaration NedZink B.V. – NedZink NOVA, NedZink NEO, NedZink NOIR
8. References
General Programme Instructions EN 15804
Institut Bauen und Umwelt e.V., Berlin (pub.): The EN 15804:2012+A2:2019
preparation of environmental product declarations Sustainability of construction works - Environmental
(EPDs); General Programme Instructions for the Product Declarations - Core rules for the product
preparation of EPDs at the Institut Bauen und Umwelt category of construction products
e.V. (IBU) V2.0, 2021
www.ibu-epd.com DIN 4102
DIN 4102
Fire behaviour of building materials and building
PCR 2021 Part A components
Institut Bauen und Umwelt e.V., Berlin: Product
Category Rules for Construction Products from the ISO 9001
range of Environmental Product Declarations of Institut ISO 9001:2015
Bauen und Umwelt (IBU), Part A: Calculation Rules for Quality management systems - Requirements
the Life Cycle Assessment and Requirements on the
Background Report according to EN 15804+A2:2019. ISO 14001
Version 1.1, January 2021 ISO 14001:2015
www.ibu-epd.com Environmental management systems - Requirements
with guidance for use
PCR 2017 Part B
Institut Bauen und Umwelt e.V., Berlin: Product ISO 14025
Category Rules for Construction Products from the ISO 14025:2011-10
range of Environmental Product Declarations of Institut Environmental labels and declarations - Type III
Bauen und Umwelt (IBU), Part B: Requirements on the environmental declarations - Principles and procedures
EPD for Building Metals. Version 1.6, November 2017
www.ibu-epd.com ISO 14040
ISO 14040:2006
EN 612 Environmental management - Life cycle assessment -
EN 612:2005 Principles and framework
Eaves gutters with bead stiffened fronts and rainwater
pipes with seamed joints made of metal sheet ISO 14044
ISO 14044:2006
EN 988 Environmental management - Life cycle assessment -
EN 988:1996 Requirements and guidelines
Zinc and zinc alloys - Specification for rolled flat
products for building ISO 15686
ISO 15686
EN 1179 Buildings and constructed assets - Service life
EN 1179:2003 planning
Zinc and zinc alloys - Primary zinc
Regulation (EU) No. 305/2011
EN 13501-1 Regulation (EU) No 305/2011 of the European
EN 13501-1:2007+A1:2009 Parliament and of the Council of 9 March 2011 laying
Fire classification of construction products and building down harmonised conditions for the marketing of
elements - Part 1: Classification using data from construction products and repealing Council Directive
reaction to fire tests 89/106/EEC (Text with EEA relevance)
EN 13501-5 96/603/EC
EN 13501-5:2006+A1:2009 EU Commission Decision of 4 October 1996
Fire classification of construction products and building establishing the list of products belonging to Classes A
elements - Part 5: Classification using data from 'No contribution to fire' provided for in Decision
external fire exposure to roofs tests 94/611/EC implementing Article 20 of Council Directive
89/106/EEC on construction products (Text with EEA
EN 14782 relevance)
EN 14782:2006
Self-supporting metal sheet for roofing, external KOMO product certificates
cladding and internal lining - Product specification and BRL2034: K7054/04 zinc sheets
requirements BRL2035: K7057/04 zinc gutters
BRL2044: K7063/04 zinc downpipes
EN 14783
EN 14783:2013 Lloyd's Register Product certificate (approval No
Fully supported metal sheet and strip for roofing, QIS 122)
external cladding and internal lining - Product Lloyd’s Register Inspection Services - Product
specification and requirements certificate Industrial Quality Scheme for Product
Certification by Surveillance of Quality Systems
(approval No QIS 122)
9 Environmental Product Declaration NedZink B.V. – NedZink NOVA, NedZink NEO, NedZink NOIR
Candidate List of substances of very high concern Zinc…A Sustainable Material
for Authorisation International Zinc Association (2010)
ECHA published in accordance with Article 59(10) of
the REACH Regulation (2018) Zinc, A Sustainable Material – Essential for Modern
Life.
Bundesinstitut für Bau-, Stadt- und International Zinc Association (2017)
Raumforschung (BBSR)
Nutzungsdauer von Bauteilen für International Zinc Association (IZA)
Lebenszyklusanalysen nach BNB (BNB: Global industry association dedicated to the interests
Bewertungssystem Nachhaltiges Bauen)(2011) of zinc and its users
www.zinc.org
TNO-MEP-99/441
Diffusive Emissions of zinc due to atmospheric SimaPro V9.0
corrosion of zinc and zinc-coated (galvanised) Life Cycle Assessment software
materials - R.H.J. Korenromp, J.C.Th. Hollander
(1999) Ecoinvent V3.6
Life Cycle Inventory database, 2019
Zinc Environmental Profile - 2015 Update
International Zinc Association (2016)
Zinc Recycling, Closing the Loop
International Zinc Association (2011)
10 Environmental Product Declaration NedZink B.V. – NedZink NOVA, NedZink NEO, NedZink NOIR
Publisher
Institut Bauen und Umwelt e.V. Tel +49 (0)30 3087748- 0
Panoramastr. 1 Fax +49 (0)30 3087748- 29
10178 Berlin Mail info@ibu-epd.com
Germany Web www.ibu-epd.com
Programme holder
Institut Bauen und Umwelt e.V. Tel +49 (0)30 - 3087748- 0
Panoramastr 1 Fax +49 (0)30 – 3087748 - 29
10178 Berlin Mail info@ibu-epd.com
Germany Web www.ibu-epd.com
Author of the Life Cycle
Assessment Tel +31 (0)30-693 00 55
Stichting Adviescentrum Metaal Fax +31 (0)30-693 00 57
Kelvinbaan 40 Mail info@metaaladvies.nl
3430MT Nieuwegein Web metaaladvies.nl
Netherlands
Owner of the Declaration
NedZink B.V. Tel +31 (0)475 455700
Hoofdstraat 1 Fax +31 (0)475 455790
6024AA Budel-Dorplein Mail info@nedzink.com
Netherlands Web www.nedzink.com
