ENVIRONMENTAL PRODUCT DECLARATION
as per ISO 14025 and EN 15804
Owner of the Declaration Kaimann GmbH
Programme holder Institut Bauen und Umwelt e.V. (IBU)
Publisher Institut Bauen und Umwelt e.V. (IBU)
Declaration number EPD-KAI-20200016-IBC1-EN
Issue date 08.06.2020
Valid to 07.06.2025
Kaiflex KKplus s2
Kaimann GmbH
www.ibu-epd.com | https://epd-online.com
Umwelt Produktdeklaration Name des Herstellers – Name des Produkts
1. General Information
Kaimann GmbH Kaiflex KKplus s2
Programme holder Owner of the declaration
IBU – Institut Bauen und Umwelt e.V. Kaimann GmbH
Panoramastr. 1 Hansastraße 2-5
10178 Berlin 33161 Hövelhof
Germany
Declaration number Declared product / declared unit
EPD-KAI-20200016-IBC1-EN 1 m3 insulation material Kaiflex KKplus s2
This declaration is based on the product Scope:
category rules: Product line Kaiflex KKplus s2
Insulating materials made of foam plastics, 06.2017 Thermal insulation material made of flexible
(PCR checked and approved by the SVR) elastomeric foam for technical building equipment and
industrial installations.
Issue date The EPD is performed in agreement with the demands
08.06.2020 of PCR Part A with reference to EN 15804+A1:2013
and PCR Part B: Requirements on the EPD for
insulating materials made of foam plastics.
Valid to
The EPD is based on the average Kaiflex KKplus s2
07.06.2025
production from two different variations produced in
Germany.
The owner of the declaration shall be liable for the
underlying information and evidence; the IBU shall not
be liable with respect to manufacturer information, life
cycle assessment data and evidences.
Verification
The standard EN 15804 serves as the core PCR
Independent verification of the declaration and data
according to ISO 14025:2010
Dipl. Ing. Hans Peters internally x externally
(chairman of Institut Bauen und Umwelt e.V.)
Dr. Alexander Röder Matthias Klingler
(Managing Director Institut Bauen und Umwelt e.V.)) (Independent verifier appointed by SVR)
2. Product
2.1 Product description/Product definition
Kaiflex KKplus s2 is a flexible closed cell rubber 2.2 Application
insulation made of flexible elastomeric foam (FEF) that Kaiflex KKplus s2 is used for air-conditioning,
prevents condensation and reduces energy loss. By refrigeration, chilled water, heating and hot water pipes
incorporating a water vapour barrier into the insulation and air-distribution ductwork. In addition to preventing
cell structure Kaiflex KKplus s2 can effectively condensation and saving energy, Kaiflex KKplus s2
eliminate water vapour migration and retain its also performs an acoustic function, absorbing sound
performance over the entire system life. This EPD and dampening duct wall vibration. With inherent anti-
covers the Kaiflex KKplus s2 product family including microbial resistance as standard, and a Class B fire
tubes and sheets. rated, closed cell rubber that is completely dust and
fibre free, Kaiflex KKplus s2 can be used in any kind of
For the placing on the market of the product in the public, commercial or industrial building without
European Union/European Trade Association impacting on health or the quality of air. Outdoor
(EU/EFTA) (with the exception of Switzerland) application requires protection against UV-radiation.
Regulation (EU) No. 305/2011 (CPR) applies. The
product needs a declaration of performance taking into 2.3 Technical Data
consideration EN 14304:2009 , Thermal insulation
products for building equipment and industrial
installations - Factory made flexible elastomeric foam Constructional data
(FEF) products - Specification, and the CE-marking. Name Value Unit
For the application and use the respective national Gross density 67.51 kg/m3
provisions apply. Water vapour diffusion resistance tube: µ ≥
-
factor acc. to EN 12088 10000, sheet:
2 Environmental Product Declaration Kaimann GmbH – Kaiflex KKplus s2
µ ≥ 7000 adhesives and stabilizers are for processing and
tube: λϑ = process control.
0.033 + 7.2 ·
10E-5 ϑ + 1) This product/article/at least one partial article
1.2*10E-7*ϑ², contains substances listed in the candidate list
Thermal conductivity W/(mK)
sheet: λϑ = (16.01.2020) exceeding 0.1 percentage by mass: no.
0.038 + 8*10E- 2) This product/article/at least one partial article
5 ϑ + 1.2*10E- contains other CMR substances in categories 1A or 1B
6 ϑ² which are not on the candidate list, exceeding 0.1
tube: 0.032, percentage by mass: no.
Thermal conductivity at -10 °C W/(mK)
sheet: 0.037 3) Biocide products were added to this construction
tube: 0.033, product or it has been treated with biocide products
Thermal conductivity at 0 °C W/(mK)
sheet: 0.038 (this then concerns a treated product as defined by the
tube: 0.034, (EU) Ordinance on Biocide Products No. 528/2012):
Thermal conductivity at 10 °C sheet: 0.039 W/(mK) no.
2.6 Manufacture
Performance data of the product in accordance with
Upon delivery, the raw materials are stored in a
the declaration of performance with respect to its
warehouse and used in the production shortly after.
essential characteristics according to EN 14304:2009
The first step in the production of Kaiflex KKplus s2 is
Thermal insulation products for building equipment and
industrial installations - Factory made flexible to mix the raw materials in a kneader and to roll out the
resulting mixture which is then cut into sheets. The flat
elastomeric foam (FEF) products - Specification
sheets are passed through an industrial cooler and
cooled off. The cooled-off sheets are granulated and
the granulates are temporarily stored at room
temperature before entering the compounding plant.
2.4 Delivery status
The EPD is declared as an average product of one
In a next step, the different types of granulates enter
plant of one manufacturer. It looks at the average
environmental performance of two product varieties the compounding plant for mixing. The resulting
elastomer compound is pushed through extruders and
from the product line Kaiflex KKplus s2. This is in
accordance with the classification rules for group 1c) carried on a conveyer belt through an industrial
from PCR Part A paragraph 5.2. The products are: furnace for foaming. After foaming, the endless sheets
are passed through an industrial cooler upon which a
continuous longitudinal cut is applied to cut sheets into
 Kaiflex KKplus s2 Tube
the right width. If applicable, adhesive coating is
 Kaiflex KKplus s2 Sheet
applied on one side of the sheets. Finally, a traverse
cut trims the continuous sheet into sheets of various
Tubes are available from dN = 7 mm to 42 mm. Sheets sizes. For the packaging, cardboard, polyethylene film,
are available from dN = 3 mm to 32 mm. Both Kaiflex polypropylene film, and wooden pallets are used.
KKplus s2 products are composed of an elastomer.
The tubes have a density of 48.35 kg/m³ and make up 2.7 Environment and health during
7.2% of the produced volume (2018). The sheets have manufacturing
a density of 69 kg/m³ and make up 92.8% of the The manufacturer of Kaiflex KKplus s2 complies with
produced volume (2018). Thus, the resulting weighted national manufacturing guidelines and regulations such
average density is 67.51 kg/m³. as the German Energy Saving Regulation (EnEV) and
the German Renewable Energy Act (EEG). In addition,
2.5 Base materials/Ancillary materials KAIMANN’s environmental management is certified in
Kaiflex KKplus s2 is based on synthetic rubber and accordance with ISO 9001/ISO 14001/ISO 50001.
consists of several components. The following table
shows the components clustered into substance 2.8 Product processing/Installation
groups: The installation of Kaiflex KKplus s2 requires basic
tools such as cutters and scissors. No additional
 Rubber and polymers: 21.01% specific protection, beyond normal protective clothes,
is required.
 Fillers and pigments: 18.03%
 Blowing agent: 8.08%
2.9 Packaging
 Vulcanisation system, additives, plasticizer: Kaiflex KKplus s2 is packaged in cardboard boxes with
3.59% polypropylene and polyethylene films in varying sizes.
 Flame retardant: 48.88% The boxes are placed on wooden EURO pallets.
 Stabilizer: 0.4%
2.10 Condition of use
Changes in materials composition of Kaiflex KKplus s2
Rubber and polymer are the base material. Fillers and during the use phase only occur in case of
pigments are for firmness and colour. The blowing extraordinary effects.
agent causes the volume increase and expansion
process during the manufacture of the product. The 2.11 Environment and health during use
vulcanisation system, additives, and plasticizer provide An odour should be considered normal. The odour will
flexibility and workability. The flame retardants ensure dissipate during use (about 4 weeks) because the cells
the fire resistance of the end-product, and the are exchanged with the air.
3 Environmental Product Declaration Kaimann GmbH – Kaiflex KKplus s2
2.12 Reference service life Kaiflex foam based insulating materials have a high
water vapour transmission resistance and thus keep
possible water vapour transmission to a minimum.
Since the use stage (B1-B7) is not fully declared, the
declaration of the reference service life is only Mechanical destruction
voluntary. Foam based insulation materials have limited
mechanical stability and low elastic modulus. Thus, it
2.13 Extraordinary effects should be externally supported if subjected to greater
mechanical loads.
Fire
Kaiflex KKplus s2 is designed to meet European fire 2.14 Re-use phase
regulations and is a self-extinguishing foam that will At the end-of-life, Kaiflex KKplus s2 can be used for
not drip or support flame spread. It can be safely used energy recovery in a waste incineration plant, as well
with confidence in public, commercial and industrial as the plastic from packaging. The cardboard and
buildings. wooden pallets from packaging can be re-used.
Fire protection 2.15 Disposal
Name Value Kaiflex KKplus s2 is disposed of in accordance with
Building material class B (sheets) / BL (tubes) local regulations governed by the European Waste
Burning droplets d0 Catalogue 2014 (waste code: 07 wastes from organic
Smoke gas development s2 chemical processes - 07 02 13 waste plastic).
Water 2.16 Further information
Additional information about Kaiflex KKplus s2 is
available on https://kaimann.com/.
3. LCA: Calculation rules
3.1 Declared Unit as well as buildings to manufacturing the declared unit
The declared unit is 1 m³ of the thermal insulation is neglected. On average, 0.49 kWh electricity and
material for technical building equipment and industrial 2.65 kWh natural gas are required for the
installations Kaiflex KKplus s2. The declared unit refers manufacturing of 1m³ Kaiflex KKplus s2. This data was
to the product as it leaves the factory gate. The gross provided by Kaimann GmbH. This module also
density is the average density of al declared products, includes packaging with plastics and cardboard and
weighted by production volume. wooden pallets. The biogenic carbon stored is
declared in the result section.
Declared unit
Name Value Unit Module A4: The transport of Kaiflex KKplus s2 from
Gross density 67.51 kg/m3 the factory gate to the site of assembly is represented
Conversion factor to 1 kg 67.51 - through generic background data. The transportation
Declared unit 1 m3 distances are based on average transportation data
provided by the manufacturer.
Module A5: The assembly can be done manually
3.2 System boundary without the use of any electrical equipment. Only glue
This EPD is a cradle-to-gate EPD with options. The (Spezialkleber) is required for the assembly of Kaiflex
system boundaries of the EPD follow the modular KKplus s2. Packaging material from module A3 is
structure of EN 15804 (according to EN 15804, section disposed of here: Plastic packaging is incinerated, and
6.2.1). Only the declaration of the product stage cardboard and the wooden pallet are re-used.
modules A1 to A3 is mandatory for compliance with EN
15804. The declaration of the modules of other life Modules B1-B7: No resource use and impacts occur
cycle stages is optional. Resources from the during the use phase of the products.
ecosphere and Technosphere enter the system on
stage A1 and leave the system on stage C4. The Modules C1&C3: Dismantling of Kaiflex KKplus s2 is
following life cycle stages are considered: done manually without using any electrical equipment.
No processing is required before disposal. Therefore,
Module A1: The system boundaries comprise raw module C1 and C3 are disregarded.
material extraction and supply from cradle to factory
gate and is represented through generic background Module C2: The products to be disposed of are
data sets. transported to the waste treatment facility.
Module A2: The transport of the raw materials from Module C4: The waste is treated according to the
the factory gate to the point of manufacturing is waste framework directive of the European Union.
represented through generic background data sets.
The transportation distances have been provided by Module D: Potential impacts and benefits from energy
the manufacturer. recovery and recycling are described.
Module A3: The manufacturing includes 3.3 Estimates and assumptions
manufacturer-specific material and energy data which The type of EPD is cradle to gate.
are represented through generic data sets. Machinery,
4 Environmental Product Declaration Kaimann GmbH – Kaiflex KKplus s2
Module A2: Raw materials are transported to the
manufacturer by road transport and shipping. 3.6 Data quality
Information on the transportation distances was The life cycle inventory for the assessed product is
provided by the manufacturer. For the calculation, the based on an internal assessment of manufacturing and
distances were weighted by the mass of the respective environmental data, assessment of LCA-relevant data
raw materials. for the supply chain and energy measurement within
the factors. The required product flows for creation of
Module A3: No production waste is assumed during the product system were handed over to GreenDelta
the production of Kaiflex. For further information, see GmbH.
chapter 5.4 Allocation. All data was scrutinised and found to be plausible and
consistent and were therefore found to be
Module A4: Kaiflex KKplus s2 is distributed worldwide. representative.
The average transportation distance per declared unit Some of the background data sets are more than 10
was calculated based on the sales volume and years old but were used when no recent dataset was
average transportation distance per country where available. Datasets from the GaBi database are
Kaiflex KKplus s2 is distributed. Whenever the country assumed to have a high quality.
was outside of Europe and the distance to the target There are no materials or processes that are left out
country was higher than 2,000 km, it was assumed that because they are under the cut-off threshold.
only 750 km of the transportation distance were
covered by road (from the manufacturer to the harbour 3.7 Period under review
and from the harbour to the point of use) whereas the The production data refers to the average of the year
rest of the distance was covered by shipping. 2018.
Distances within Europe or shorter than 2,000 km are
assumed to be covered fully by road. Based on the 3.8 Allocation
sum product of sales volume multiplied with the road No allocation is carried out.
and ship transportation, the total transportation
distances were calculated and divided by the total 3.9 Comparability
sales volume to calculate the average transportation Basically, a comparison or an evaluation of EPD data
distance per declared unit. As a result, the average is only possible if all the data sets to be compared
road transportation distance per declared unit is 573 were created according to EN 15804 and the building
kilometres by road and 228 kilometres by ship. No loss context, respectively the product-specific
during transportation is assumed. characteristics of performance, are taken into account.
Module A5: As a background database GaBi database
Kaiflex KKplus s2 is assembled by manual labour professional database (version from September 2019)
under use of adhesive. It is assumed that no further by thinkstep AG was used and has been
energy or materials are required in this module (apart complemented by data sets from GaBi extension
from the manual labour and adhesive), and that databases as well as data sets from the EuGeos
consumers of Kaiflex KKplus s2 order correct product database version 2.1 by EuGeos Ltd.
sizes and thus avoid waste production during the
assembly. The packaging materials are disposed of by
re-using (cardboard and wooden pallet) and by
incineration (polyethylene and polypropylene).
Module C2: The average distance of disassembled
Kaiflex KKplus s2 to the point of disposal is assumed
to be 75 kilometres covered by road.
Module C4: Kaiflex KKplus s2 is incinerated.
3.4 Cut-off criteria
All material flows in module A1 are covered and almost
all material and energy flows in module A3 are
covered. Neglected material or energy flows have a
mass or energy contribution of less than one percent
per process and contribute to less than 5% of mass
and energy flows of a module. Infrastructure such as
office buildings and the manufacturing hall as well as
the machinery required to produce Kaiflex KKplus s2
have not been considered.
3.5 Background data
The LCA model underlying this EPD was created in
openLCA 1.10 developed by GreenDelta GmbH. As a
background database GaBi database professional
database (version from September 2019) by thinkstep
AG was used and has been complemented by data
sets from GaBi database extension databases as well
as data sets from the EuGeos database version 2.1 by
EuGeos Ltd.
5 Environmental Product Declaration Kaimann GmbH – Kaiflex KKplus s2
4. LCA: Scenarios and additional technical information
The following technical scenario information serves as
a basis for the declared modules. All values refer to the
declared unit of 1 m³.
Transport to the building site (A4)
Name Value Unit
Transport distance (road) 573 km
transport distance (ship) 228 km
Installation into the building (A5)
Name Value Unit
Auxiliary 1.6 kg
Water consumption 0 m3
Other resources 0 kg
Electricity consumption 0 kWh
Other energy carriers 0 MJ
Material loss 0 kg
Output substances following
16.5 kg
waste treatment on site
Dust in the air 0 kg
VOC in the air 0 kg
The 16.5 kg are the sum of all packaging materials per
declared unit.
End of life (C1-C4)
Name Value Unit
Collected separately 69.11 kg
Collected as mixed construction
0 kg
waste
Reuse 0 kg
Recycling 0 kg
Energy recovery 69.11 kg
Landfilling 0 kg
67.51 kg Kaiflex and 1.6 kg Kaiflex Spezialkleber are
incinerated for energy recovery.
Reuse, recovery and/or recycling potentials (D),
relevant scenario information
Module D includes the credits from the material re-use
in module A5 and the credits of the incineration
processes from A5 (packaging waste) and C4 at a
waste incineration plant with an assumed efficiency of
R1<0.6.
6 Environmental Product Declaration Kaimann GmbH – Kaiflex KKplus s2
5. LCA: Results
The life cycle impact assessment method is based on EN15804. Energy indicators for resource use utilise the
lower calorific value.
DESCRIPTION OF THE SYSTEM BOUNDARY (X = INCLUDED IN LCA; MND = MODULE NOT DECLARED;
MNR = MODULE NOT RELEVANT)
BENEFITS AND
CONSTRUCTI LOADS
PRODUCT STAGE ON PROCESS USE STAGE END OF LIFE STAGE BEYOND THE
STAGE SYSTEM
BOUNDARIES
7 Environmental Product Declaration Kaimann GmbH – Kaiflex KKplus s2
lairetam
waR
ylppus tropsnarT
gnirutcafunaM
eht
morf
tropsnarT
etis
eht
ot
etag
ylbmessA esU
ecnanetniaM
riapeR
tnemecalpeR tnemhsibrufeR
ygrene
lanoitarepO esu
retaw
lanoitarepO esu
noitcurtsnoc-eD
noitilomed tropsnarT
gnissecorp
etsaW
lasopsiD -esueR -yrevoceR -gnilcyceR laitnetop
A1 A2 A3 A4 A5 B1 B2 B3 B4 B5 B6 B7 C1 C2 C3 C4 D
X X X X X MND MND MNR MNR MNR MND MND MND X MND X X
RESULTS OF THE LCA - ENVIRONMENTAL IMPACT: 1 m³
Param
Unit A1 A2 A3 A4 A5 C2 C4 D
eter
GWP [kg CO2-Eq.] 2.22E+2 1.09E+1 2.64E+1 6.54E+0 1.18E+1 8.27E-1 1.75E+2 -1.93E+2
ODP [kg CFC11-Eq.] 4.29E-5 5.38E-7 2.23E-7 1.18E-6 5.09E-7 1.54E-7 1.21E-13 -2.23E-7
AP [kg SO2-Eq.] 1.38E+0 2.40E-1 8.69E-2 3.13E-2 1.48E-2 3.27E-3 1.98E-2 -1.92E-1
EP [kg (PO4)3--Eq.] 9.04E-1 2.71E-2 2.05E-2 6.56E-3 5.99E-3 7.70E-4 4.62E-3 -4.69E-2
POCP [kg ethene-Eq.] 5.54E-2 6.83E-3 5.07E-3 1.22E-3 2.54E-3 1.36E-4 1.17E-3 -9.83E-3
ADPE [kg Sb-Eq.] 3.42E-2 8.86E-6 9.33E-6 1.90E-5 1.11E-5 2.48E-6 1.17E-6 -1.25E-5
ADPF [MJ] 4.05E+3 1.42E+2 3.19E+2 1.00E+2 9.22E+1 1.28E+1 7.28E+1 -1.48E+3
GWP = Global warming potential; ODP = Depletion potential of the stratospheric ozone layer; AP = Acidification potential of land and water; EP =
Caption Eutrophication potential; POCP = Formation potential of tropospheric ozone photochemical oxidants; ADPE = Abiotic depletion potential for non-
fossil resources; ADPF = Abiotic depletion potential for fossil resources
RESULTS OF THE LCA - RESOURCE USE: 1 m³
Parameter Unit A1 A2 A3 A4 A5 C2 C4 D
PERE [MJ] 2.86E+2 8.84E-1 2.79E+2 1.29E+0 6.71E+0 1.68E-1 2.04E+1 -4.94E+2
PERM [MJ] 0.00E+0 0.00E+0 2.35E+2 0.00E+0 0.00E+0 0.00E+0 0.00E+0 -2.35E+2
PERT [MJ] 2.86E+2 8.84E-1 5.13E+2 1.29E+0 6.71E+0 1.68E-1 2.04E+1 -7.29E+2
PENRE [MJ] 1.37E+3 1.42E+2 2.24E+2 1.02E+2 2.10E+2 1.30E+1 2.94E+3 -1.48E+3
PENRM [MJ] 2.86E+3 0.00E+0 1.16E+2 0.00E+0 -1.16E+2 0.00E+0 -2.86E+3 0.00E+0
PENRT [MJ] 4.24E+3 1.42E+2 3.40E+2 1.02E+2 9.41E+1 1.30E+1 7.28E+1 -1.48E+3
SM [kg] 0.00E+0 0.00E+0 0.00E+0 0.00E+0 0.00E+0 0.00E+0 0.00E+0 0.00E+0
RSF [MJ] 0.00E+0 0.00E+0 0.00E+0 0.00E+0 0.00E+0 0.00E+0 0.00E+0 0.00E+0
NRSF [MJ] 0.00E+0 0.00E+0 0.00E+0 0.00E+0 0.00E+0 0.00E+0 0.00E+0 0.00E+0
FW [m³] 5.50E+0 1.32E-2 7.24E-1 1.88E-2 1.10E-1 2.44E-3 5.70E-1 -3.41E+0
PERE = Use of renewable primary energy excluding renewable primary energy resources used as raw materials; PERM = Use of
renewable primary energy resources used as raw materials; PERT = Total use of renewable primary energy resources; PENRE = Use of
non-renewable primary energy excluding non-renewable primary energy resources used as raw materials; PENRM = Use of non-
Caption
renewable primary energy resources used as raw materials; PENRT = Total use of non-renewable primary energy resources; SM = Use
of secondary material; RSF = Use of renewable secondary fuels; NRSF = Use of non-renewable secondary fuels; FW = Use of net fresh
water
RESULTS OF THE LCA – OUTPUT FLOWS AND WASTE CATEGORIES:
1 m³
Parameter Unit A1 A2 A3 A4 A5 C2 C4 D
HWD [kg] 2.95E-2 1.04E-8 9.50E-3 2.88E-10 4.01E-8 0.00E+0 4.50E-7 -1.70E-3
NHWD [kg] 1.40E+2 2.04E-1 9.01E+0 5.64E-3 4.08E+0 0.00E+0 5.13E+1 -2.76E+2
RWD [kg] 2.80E-2 1.17E-4 2.79E-3 3.22E-6 7.24E-4 0.00E+0 3.48E-3 -4.56E-3
CRU [kg] 0.00E+0 0.00E+0 0.00E+0 0.00E+0 1.37E+1 0.00E+0 0.00E+0 0.00E+0
MFR [kg] 0.00E+0 0.00E+0 0.00E+0 0.00E+0 0.00E+0 0.00E+0 0.00E+0 0.00E+0
MER [kg] 0.00E+0 0.00E+0 0.00E+0 0.00E+0 0.00E+0 0.00E+0 0.00E+0 0.00E+0
EEE [MJ] 0.00E+0 0.00E+0 0.00E+0 0.00E+0 0.00E+0 0.00E+0 0.00E+0 0.00E+0
EET [MJ] 0.00E+0 0.00E+0 0.00E+0 0.00E+0 6.94E+1 0.00E+0 1.72E+3 0.00E+0
HWD = Hazardous waste disposed; NHWD = Non-hazardous waste disposed; RWD = Radioactive waste disposed; CRU = Components
Caption for re-use; MFR = Materials for recycling; MER = Materials for energy recovery; EEE = Exported electrical energy; EEE = Exported
thermal energy
Additional Technical scenario:
Biogenic carbon is not included in the results. It enters the product system with wood and cardboard in modules
A3 and is ‘released’ by being an avoided burden in module A5 (declared in module D) and has thus no net-effect
on the overall results. The wooden pallet has approximately 23 kg biogenic CO , and the carboard has 16 kg.
2
6. LCA: Interpretation
Environmental Impacts
The most secondary materials are used to produce the
blowing agent.
All seven environmental impact categories are
dominated by module A1 raw material supply. For six Use of net fresh water (FW)
of them, the production of the blowing agent is the This impact category is dominated by module A1 raw
largest contributor. material supply.
The production of the blowing agent uses the most
Renewable primary energy as energy carrier fresh water.
(PERE)
This impact category is dominated by the module A3 Hazardous waste disposed (HWD)
manufacturing. This impact category is dominated by modules A1 raw
Most of the renewable energy is used in the production material supply and A2 transport.
process of the EURO pallet and the cardboard. Most of the hazardous waste comes from the
production of the blowing agent for A1 and the fuel for
Renewable primary energy resources as material A2.
utilization (PERM)
The dominant modules are A3 manufacturing and the Non-hazardous waste disposed (NHWD)
avoided burdens in module D. This impact category is dominated by module A1 raw
Most of the renewable energy is stored in the wood of material supply.
the EURO pallet and is ‘released’ in module D because The main contributors are the production of the base
of re-using. material and the flame-retardant.
Non-renewable primary energy as energy carrier Radioactive waste disposed (RWD)
(PENRE) This impact category is dominated by module A1 raw
The dominant module is A2 because of the long material supply.
transport distances and A3 assembly. Most radioactive waste stems from the production of
Fuel is the main contributor to the transport. the base material, the blowing agent, and the base
material.
Non-renewable primary energy as material
utilization (PENRM) Materials for recycling (MFR)
The dominant module is A1 raw material supply, where The lorry transport process includes recycling
energy is stored in the product itself. materials, mainly to produce trucks and roads. So, the
transport modules show the highest impacts in this
Use of secondary material (SM) category.
The largest contributor is the module A1 raw material
supply.
8 Environmental Product Declaration Kaimann GmbH – Kaiflex KKplus s2
Conclusion
The production of the blowing agent is the largest
contributor to the environmental impacts of Kaiflex
KKplus s2.
7. Requisite evidence
Carcinogenic Substances <1 μg/m3
7.1 VOC emissions
The Volatile Organic Compound (VOC) emissions AgBB overview of results (3 days [µg/m³])
have been tested by Eurofins Product Testing A/S by Name Value Unit
using the Committee for health-related evaluation of TVOC (C6 - C16) <5 μg/m3
building products/Deutsches Institut für Bautechnik Sum SVOC (C16 - C22) <5 μg/m3
(AgBB/DIBt) test method in 09.2013. R (dimensionless) <1 -
VOC without NIK <5 μg/m3
AgBB overview of results (28 days [µg/m³]) Carcinogenic Substances <1 μg/m3
Name Value Unit
TVOC (C6 - C16) <5 μg/m3
7.2 Leaching performance
Sum SVOC (C16 - C22) <5 μg/m3
The concentration of water-soluble chloride ions is 300
R (dimensionless) <1 - mg/kg according to EN 13468:2001.
VOC without NIK <5 μg/m3
8. References
AGBB/DIBt
Deusches Institut für Bautechnik 2018: Anforderungen ISO 9001
an die Innenraumluftqualität in Gebäuden: ISO 9001:2015, Quality management systems -
Gesundheitliche Bewertung der Emissionen von Requirements
flüchtigen organischen Verbindungen (VVOC, VOC
und SVOC) aus Bauprodukten ISO 14001
ISO 14001:2015-0/, Environmental management
EN 12088 systems - Requirements with guidance for use
EN 12088:2013, Thermal insulating products for
building applications. Determination of long term water ISO 50001
absorption by diffusion ISO 50001:2018-08, Energy management systems -
Requirements with guidance for use
EN 13468
EN 13468:2001, Thermal insulating products for openLCA 1.10
building equipment and industrial installations - open LCA 1.10.2 (2020), Sustainability Software,
Determination of trace quantities of water soluble Databases, and Consulting. Developed by GreenDelta
chloride, fluoride, silicate, and sodium ions and pH GmbH. http://www.openlca.org/
EN 14304 PCR Part A
EN 14304:2009+A1:2013, Thermal insulation products PCR Part A Version 1.8, Calculation Rules for the Life
for building equipment and industrial installations - Cycle Assessment and Requirements on the Project
Factory made flexible elastomeric foam (FEF) Report
products - Specification
PCR Part B
EN 15804 PCR Part B Version 1.6, Requirements on the EPD for
EN 15804:2012+A1:2013, Nachhaltigkeit von insulating materials made of foam plastics
Bauwerken – Umweltproduktdeklarationen –
Grundregeln für die Produktkategorie Bauprodukte REACH 2006
REGULATION (EC) No 1907/2006 OF THE
EuGeos database EUROPEAN PARLIAMENT AND OF THE COUNCIL
LCA database by EuGeos Limited concerning the Registration, Evaluation, Authorisation
and Restriction of Chemicals (REACH)
Eurofins
Eurofins Product Testing A/S, Galten, Denmark SVHC 2019
Candidate List of substances of very high concern for
European waste catalogue 2014 Authorisation (SVHC), European Chemicals Agency,
COMMISSION DECISION amending Decision Helsinki, Finland
2000/532/EC on the list of waste pursuant to Directive
2008/98/EC of the European Parliament and of the thinkstep AG
Council Sustainability Software, Data and Consulting
GABI database
LCA database SP 39. thinkstep AG. Echterdingen
2019
9 Environmental Product Declaration Kaimann GmbH – Kaiflex KKplus s2
Publisher
Institut Bauen und Umwelt e.V. Tel +49 (0)30 3087748- 0
Panoramastr. 1 Fax +49 (0)30 3087748- 29
10178 Berlin Mail info@ibu-epd.com
Germany Web www.ibu-epd.com
Programme holder
Institut Bauen und Umwelt e.V. Tel +49 (0)30 - 3087748- 0
Panoramastr 1 Fax +49 (0)30 – 3087748 - 29
10178 Berlin Mail info@ibu-epd.com
Germany Web www.ibu-epd.com
Author of the Life Cycle
Assessment Tel +49 30 6292 4320
GreenDelta GmbH Fax -
Kaiserdamm 13 Mail gd@greendelta.com
14057 Berlin Web https://www.greendelta.com
Germany
Owner of the Declaration
Kaimann GmbH Tel +49 5257 98 50 - 0
Hansastraße 2-5 Fax +49 5257 98 50 590
33161 Hövelhof Mail info@kaimann.de
Germany Web https://www.kaimann.com
