ENVIRONMENTAL PRODUCT DECLARATION
as per ISO 14025 and EN 15804+A2
Owner of the Declaration Knauf Ceiling Solutions GmbH & Co. KG
Publisher Institut Bauen und Umwelt e.V. (IBU)
Programme holder Institut Bauen und Umwelt e.V. (IBU)
Declaration number EPD-KNA-20220029-IBD2-EN
Issue date 30.03.2022
Valid to 29.03.2027
Metal Ceiling Membranes (0.7 mm, without acoustic infill)
Knauf Ceiling Solutions GmbH & Co. KG
www.ibu-epd.com | https://epd-online.com
1. General Information
Knauf Ceiling Solutions GmbH & Co. KG Metal Ceiling Membranes (0.7 mm, without
acoustic infill)
Programme holder Owner of the declaration
IBU – Institut Bauen und Umwelt e.V. Knauf Ceiling Solutions GmbH & Co. KG
Hegelplatz 1 Elsenthal 15
10117 Berlin 94481 Grafenau
Germany Germany
Declaration number Declared product / declared unit
EPD­KNA­20220029­IBD2­EN 1 m² average steel ceiling membrane with a thickness of 0.7 mm and a
surface weight of 6.70 kg/m² (no acoustic infill)
This declaration is based on the product category rules: Scope:
Metal ceilings, 01.08.2021 This document refers to average steel ceiling membranes with a thickness
(PCR checked and approved by the SVR) of 0.7 mm and a surface weight of 6.70 kg/m² (no acoustic infill).
The products are manufactured at the following production sites of Knauf
Issue date Ceiling Solutions GmbH & Co. KG:
­ Rankweil (Austria)
30.03.2022
­ Stafford (United Kingdom)
The owner of the declaration shall be liable for the underlying information
and evidence; the IBU shall not be liable with respect to manufacturer
Valid to
information, life cycle assessment data and evidences.
29.03.2027
The EPD was created according to the specifications of EN 15804+A2. In
the following, the standard will be simplified as EN 15804.
Verification
The standard EN 15804 serves as the core PCR
Independent verification of the declaration and data according to ISO
14025:2011
internally X externally
Dipl.­Ing. Hans Peters
(Chairman of Institut Bauen und Umwelt e.V.)
Florian Pronold Matthias Schulz,
(Managing Director Institut Bauen und Umwelt e.V.) (Independent verifier)
1 Environmental Product Declaration ­ Knauf Ceiling Solutions GmbH & Co. KG ­ Metal Ceiling Membranes (0.7 mm, without acoustic infill)
2. Product
reprotoxic (CMR) substances in categories 1A or 1B which are
2.1 Product description/Product definition not on the candidate list, exceeding 0.1 percentage by mass':
Knauf Ceiling Solutions metal ceiling systems are made from No.
punched and formed galvanised steel, as comprehensive
construction kits or individual components and industrially 3) 'Biocide products were added to this construction product or
manufactured. The construction kit comprises the visible it has been treated with biocide products (this then concerns a
membrane and the substructure. The membranes (tiles, panels, treated product as defined by the (EU) Ordinance on Biocide
baffles, bulkheads) are offered with various edge details and Products No. 528/2012': No.
delivered unperforated or with a range of perforation patterns,
fulfilling the functional requirements. The substructure is either 2.6 Manufacture
exposed or concealed. The system components for metal ceilings are manufactured in
a continuous manufacturing process. The sheet steel comes
For the placing on the market of the product in the European mainly in coils, gets optionally perforated, afterwards cut to
Union/European Free Trade Association (EU/EFTA) (with the size, punched, formed and powder­coated after the cleaning
exception of Switzerland) Regulation (EU) No. 305/2011 (CPR) process. Punching and perforation waste is gathered, collected
applies. The product needs a declaration of performance taking by local disposal companies, and redirected to the recycling
into consideration EN 13964:2014, suspended ceiling centres. All production steps are carried out in accordance with
requirements and test methods and the CE­marking and the requirements and test guidelines outlined in EN 13964.
UKCA­marking (in the UK).
For the application and use the respective national provisions The manufacturing plants are certified according to ISO 9001
apply. and ISO 14001.
2.2 Application 2.7 Environment and health during manufacturing
The described metal solutions are typically used internally as Manufacturing conditions do not demand any particular health
design elements, to cover the ceiling void, as well as acoustic protection measures with the exception of those designated by
solutions for sound absorption and sound attenuation, for fire the authorities for special working areas, e.g., high­visibility
resistance and against fire spreading, for cleanrooms and high vests, ear protection, safety shoes.
hygiene requirements. The threshold limit values are not exceeded at any point in the
production process. Waste emissions generated during
2.3 Technical Data production are cleaned in accordance with statutory
Metal membranes are regulated by EN 13964 and have requirements. Emissions are below those outlined in the
corresponding labelling and declaration of performance. The Technical Guidelines governing Air. Water/ground: No
following data provide an overview of results: contamination of water or soil occurs. All the values established
Constructional data inside and outside the production facilities are below the
applicable requirements governing noise protection in the UK
Name Value Unit
and Austria. Noise­intensive plant components such as
Sound absorption coefficient (ISO 354, ISO ≤
% perforation lines are isolated accordingly by structural
11654) 0.45(L)
measures. ISO 14001 certificates and other manufacturer­
Airborne sound reduction (EN 20140­9, ISO specific documents on environment protection can be
≤ 44 dB
140­3) requested from the manufacturer.
Grammage 6.7 kg/m2
2.8 Product processing/Installation
Release of formaldehyde (EN 13964) E1 ­
There are no recognised systemic hazards associated with the
Durability class (EN 13964) B ­
installation of ceiling membranes. Metal ceiling membranes are
Further characteristics according to the PCR are not relevant suspended by a substructure. Installation must be carried out
for this product. by trained personnel. Workers should wear appropriate
personal protective equipment. Equipment such as gloves and
The performance data of the product, with respect to its goggles are recommended to prevent skin irritation.
essential characteristics, is in accordance with the declaration
2.9 Packaging
of performance according to EN 13964:2014, suspended
ceiling requirements and test methods. The membranes are packaged in cardboard boxes with a
separation paper protecting the visible surface or sealed with
2.4 Delivery status transparent polyethylene film. These packages lie on
The metal ceiling systems, construction kits and components chemically untreated wooden pallets and are easily separable.
are produced in individual module sizes and can be supplied The pallets are wrapped with polyethylene stretch film. Film,
with or without substructures. Packaging is usually on pallets paper and wood can be recycled in the usual ways.
and/or in cardboard.
2.10 Condition of use
2.5 Base materials/Ancillary materials Long service life is based on regular maintenance, care and
Name Value Unit repair of the product. When handled properly, the mechanical
and structural physical properties of the metal membranes
Galvanised steel > 98 %
remain intact throughout its entire service life. Generally, the
Surface coating < 2 %
material composition of the product does not alter during the
1) 'This product contains substances listed in the candidate list period of use.
(08.07.2021) exceeding 0.1 percentage by mass': No.
2.11 Environment and health during use
2) 'This product contains other carcinogenic, mutagenic,
2 Environmental Product Declaration ­ Knauf Ceiling Solutions GmbH & Co. KG ­ Metal Ceiling Membranes (0.7 mm, without acoustic infill)
There are no known interactions between the product, the
environment and health. Volatile organic compounds are below Water
the valuation limit. No environmental influences are known in the case of
unforeseen water ingress. The resistance of the ceiling system
2.12 Reference service life following the impact of water is dependent on the corrosion
The service life of the metal membranes is for more than 50 protection class in which the ceiling system is classified.
years, depending on the area of use, exposure and state of
maintenance. Within the framework of the conditions of use, no Mechanical destruction
ageing effects are to be expected apart from visual In the case of mechanical destruction, all substances remain
discolouration caused by air circulation. bound. It can be assumed that in the case of coated ceilings,
possible paint splinters arise in such small volumes that no
2.13 Extraordinary effects
negative effects are incurred by the environment.
Fire
The declared products are classified in the fire reaction class 2.14 Re-use phase
A1 or A2­s1, d0 according to EN 13501-1. This means that they The metal ceiling systems can be removed and re­used without
are "non­combustible" according to the German building damaging the product. Metal membrane components and
authority designation (and also many other European countries) substructure components made of steel can be redirected to
with negligible smoke development and no burning droplets in material recycling.
the event of a fire.
2.15 Disposal
Fire reaction
In accordance with the Waste Index Act (AVV) and the
Name Value
European Waste Catalogue (EWC), the waste key for steel as a
Building material class A1 or A2 component of metal ceiling systems made of steel is: 17­04­05
Burning droplets s1 – Iron and steel.
Smoke gas development d0
2.16 Further information
Further information at www.knaufceilingsolutions.com
3. LCA: Calculation rules
3.1 Declared Unit 3.2 System boundary
This EPD refers to a declared unit of 1 m² of average steel The life cycle assessment of average metal ceiling membranes
ceiling membrane with a thickness of 0.7 mm (Standard white includes a cradle­to­gate analysis of the products'
RAL 9010) and a surface weight of 6.70 kg/m² without acoustic environmental impacts with modules C1–C4 and module D
infill. (A1–A3, + C + D). Subsequent life cycle phases are part of the
analysis:
Declared unit
Name Value Unit
Module A1-A3 | Production stage
Declared unit 1 m2 The production stage includes the upstream burdens of raw
Grammage 6.7 kg/m2 material supply, their transports and the manufacturing plants of
Knauf Ceiling Solutions located in Rankweil (AT) and Stafford
The production of the associated gaskets is declared in a
(UK). The production of metal ceiling membranes includes
separate annexe to this EPD.
punching, stamping and trimming, powder coating and
The substructure is not part of this EPD.
packaging. Main raw material inputs, therefore, refer to steel
and paint for powder coating. Both production sites are
The ceiling membranes are produced under different brand
supplied with electricity from the national grid and thermal
names, at the Knauf Ceiling Solutions production sites in
energy from natural gas.
Rankweil (AT) and Stafford (UK). The declared product
The packaging of the products is considered in this stage.
represents a weighted average of the two production sites
leading to a high representativity of the results.
Module C1 | Deconstruction and demolition
Disassembly of the product is done either manually or using
Knauf Ceiling Solutions metal ceiling membranes can be
smaller tools. Referring energy demand is considered to be
specifically configurated based on the customer's need
negligible.
resulting in more than 100 standard products. The declared
unit, therefore, refers to a representative product sold in large
Module C2 | Transport to disposal
quantities. All products are available in various perforation
The transport to the disposal of the material is estimated
designs. Ensuring a consistent representation the standard
declaring a 50 km radius to the disposal. In reality, this scenario
perforation of 20 % representing the major production
may vary depending on the actual location of deconstruction
quantities is declared in this EPD (specific weight without
and referring waste treatment.
perforation: 8.04 kg/m²). This approach ensures the applicability
of the EPD for specific products as well as the representativity
Module C3 | Waste processing
of the results.
Regarding the steel fraction, the material flow reaching module
D for recycling is declared as material for recycling in Module
As the mass of steel represents the decisive factor in the
C3. Environmental impacts resulting from the grinding and
product's environmental profile, a linear correlation of product
sorting of steel scrap are not included, as referring energy
mass and environmental impact is to be expected. The surface
demand is considered to be negligible. In addition, a loss rate
weight of the ceiling membranes directly depends on the
of 5 % of the processed material is assumed. 95 % of the
perforation type. Thus, the recalculation for specific perforations
material can potentially be recycled.
based on the product mass is possible.
3 Environmental Product Declaration ­ Knauf Ceiling Solutions GmbH & Co. KG ­ Metal Ceiling Membranes (0.7 mm, without acoustic infill)
Module C4 | Disposal representativeness of the database was kept in mind when
Module C4 refers to the emissions from the disposal of the selecting background data. Whenever specific data were
losses from waste processing of lost steel. The chosen missing, either generic datasets or representative average data
scenario, therefore, includes the environmental burdens of were used instead. The implemented GaBi background
landfilling of 5 % of the metal material. datasets refer to the latest versions available (not more than
ten years old) and are carefully chosen.
Module D | Benefits and loads beyond the system
boundary 3.7 Period under review
Module D declares the recycling of the recovered steel (95 % of Foreground data were collected for the production year 2020.
the product). It includes the potential for substituting primary The data are based on the volumes produced on an annual
steel. basis.
3.3 Estimates and assumptions 3.8 Geographic Representativeness
Assumptions and approximations are applied in case of a lack Land or region, in which the declared product system is
of representative data. All assumptions and approximations are manufactured, used or handled at the end of the product´s
documented precisely and represent a best­guess lifespan: Europe
representation of reality. In case of uncertainty, a conservative
approach is chosen.
3.9 Allocation
3.4 Cut-off criteria For foreground data, the calculation of specific input quantities
The LCA model covers all available input and output flows, is based on the annual production quantity (square meter), e.g.
which can be represented based on robust data. Data gaps are for energy input, packaging, etc.. The steel input on product
filled with conservative assumptions from average data (when level was calculated based on the mass of steel in the output.
available) or with generic data and are documented
accordingly. Only data with a contribution lower than 1 % were Background data for the supply chain of the steel are published
cut off. Thus, no data were neglected, of which a substantial by worldsteel (GaBi-databases). Representing an average of
impact is to be expected. All relevant data were collected the global steel industry, worldsteel background datasets
comprehensively. Cut­off material and energy flows were ensure a good geographical and technological representation
chosen carefully based on their expected quantitative of steel production. All worldsteel datasets are modelled
contribution as well as potential environmental impacts. Thus, it according to the worldsteel LCA methodology, applying the
can be assumed that the sum of all neglected input flows does system expansion approach for the allocation of co­products
not account for more than 5 % of the total material, water and from steel production. As a result, these datasets are not fully
energy flows. compliant with the requirements of the EN 15804, which
emphasises the so­called partitioning approach applying a
3.5 Background data subdivision of environmental impacts according to their physical
This study uses generic background data for the evaluation of relationships. Due to a lack of global data calculated based on
upstream environmental impacts from GaBi databases (GaBi the partitioning approach, the worldsteel datasets refer to the
10; 2021.2). closest representation of steel production in this context.
Additionally, the deviation of the results of the two allocation
3.6 Data quality approaches is to be expected under 5 % according to Sphera.
Data collection is based on product­specific questionnaires. It Scrap input is regarded as burden­free.
follows an iterative process clarifying questions via e­mail,
telephone calls or in personal/web meetings. Intensive 3.10 Comparability
discussions between Knauf Ceiling Solutions and Daxner & Basically, a comparison or an evaluation of EPD data is only
Merl results in an accurate mapping of product­related material possible if all the data sets to be compared were created
and energy flows. This leads to a high quality of foreground according to EN 15804 and the building context, respectively
data collected. Data collection relies on a consistent process the product­specific characteristics of performance, are taken
according to ISO 14044. into account.
The GaBi background database was used to calculate the LCA
The technological, geographical and time­related (GaBi 10; 2021.2).
4. LCA: Scenarios and additional technical information
End of life (C1-C4)
Characteristic product properties of biogenic carbon
Name Value Unit
Information on describing the biogenic Carbon Content at
Collected separately (steel) 6.7 kg
factory gate
Recycling 95 % 6.37 kg
Name ValueUnit
Landfilling 5 % 0.33 kg
Biogenic carbon content in accompanying kg
0.1
packaging C
Reuse, recovery and/or recycling potentials (D), relevant
The declared product does not contain biogenic carbon. scenario information
Name Value Unit
Net flow of steel scrap 7.66 kg/m²
4 Environmental Product Declaration ­ Knauf Ceiling Solutions GmbH & Co. KG ­ Metal Ceiling Membranes (0.7 mm, without acoustic infill)
5. LCA: Results
The following table contains the LCA results for a declared unit of 1 m² average steel ceiling membrane with a thickness of 0.7 mm and
a surface weight of 6.70 kg/m² (no acoustic infill).
Disclaimer:
EP­freshwater: This indicator has been calculated as 'kg P eq' as required in the characterization model (EUTREND model, Struijs et
al., 2009b, as implemented in ReCiPe; http://eplca.jrc.ec.europa.eu/LCDN/developerEF.xhtml).
DESCRIPTION OF THE SYSTEM BOUNDARY (X = INCLUDED IN LCA; ND = MODULE OR INDICATOR NOT DECLARED; MNR =
MODULE NOT RELEVANT)
Benefits and
Construction loads beyond
Product stage Use stage End of life stage
process stage the system
boundaries
la ire ta m w a Ry lp p u s tro p s n a rT g n iru tc a fu n a M e h t m o rf tro p s n a rTe tis e h t o t e ta g y lb m e s s A e s U e c n a n e tn ia M ria p e R tn e m e c a lp e R tn e m h s ib ru fe R y g re n e la n o ita re p Oe s u re ta w la n o ita re p Oe s u n o itc u rts n o c ­e Dn o itilo m e d tro p s n a rT g n is s e c o rp e ts a W la s o p s iD ­e s u e R­y re v o c e R­g n ilc y c e Rla itn e to p
A1 A2 A3 A4 A5 B1 B2 B3 B4 B5 B6 B7 C1 C2 C3 C4 D
X X X MND MND MND MND MNR MNR MNR MND MND X X X X X
RESULTS OF THE LCA - ENVIRONMENTAL IMPACT according to EN 15804+A2: 1 m² ceiling membrane (0.7 mm; 6.70 kg/m²)
Parameter Unit A1-A3 C1 C2 C3 C4 D
Global Warming Potential total (GWP­total) kg CO 2 eq 2.59E+01 0 2.03E­02 0 1.62E­02 ­1.3E+01
Global Warming Potential fossil fuels (GWP­fossil) kg CO 2 eq 2.62E+01 0 2.01E­02 0 1.64E­02 ­1.3E+01
Global Warming Potential biogenic (GWP­biogenic) kg CO 2 eq ­2.21E­01 0 ­2.39E­05 0 ­1.68E­04 ­7.41E­03
Global Warming Potential luluc (GWP­luluc) kg CO 2 eq 1.23E­02 0 1.64E­04 0 1.64E­05 ­2.85E­04
Depletion potential of the stratospheric ozone layer (ODP) kg CFC11 eq 2.54E­12 0 3.95E­18 0 3.86E­17 ­3.1E­14
Acidification potential of land and water (AP) mol H+ eq 6.42E­02 0 6.64E­05 0 5.21E­05 ­2.32E­02
Eutrophication potential aquatic freshwater (EP­freshwater) kg P eq 3.24E­05 0 5.95E­08 0 1.25E­08 ­2.83E­06
Eutrophication potential aquatic marine (EP­marine) kg N eq 1.62E­02 0 3.05E­05 0 1.29E­05 ­4.47E­03
Eutrophication potential terrestrial (EP­terrestrial) mol N eq 1.72E­01 0 3.41E­04 0 1.42E­04 ­4.52E­02
Formation potential of tropospheric ozone photochemical oxidants kg NMVOC
5.33E­02 0 5.99E­05 0 4.08E­05 ­2E­02
(POCP) eq
Abiotic depletion potential for non fossil resources (ADPE) kg Sb eq 1.15E­04 0 1.78E­09 0 1.13E­09 ­3.23E­05
Abiotic depletion potential for fossil resources (ADPF) MJ 2.94E+02 0 2.67E­01 0 2.38E­01 ­1.27E+02
m3 world eq
Water use (WDP) 1.09E+01 0 1.86E­04 0 ­1.94E­04 ­3.55E+01
deprived
RESULTS OF THE LCA - INDICATORS TO DESCRIBE RESOURCE USE according to EN 15804+A2: 1 m² ceiling membrane (0.7
mm; 6.70 kg/m²)
Parameter Unit A1-A3 C1 C2 C3 C4 D
Renewable primary energy as energy carrier (PERE) MJ 2.63E+01 0 1.54E­02 0 1.72E­02 8.01E+00
Renewable primary energy resources as material utilization
MJ 3.73E+00 0 0 0 0 0
(PERM)
Total use of renewable primary energy resources (PERT) MJ 3.01E+01 0 1.54E­02 0 1.72E­02 8.01E+00
Non renewable primary energy as energy carrier (PENRE) MJ 2.84E+02 0 2.68E­01 0 2.38E­01 ­1.27E+02
Non renewable primary energy as material utilization (PENRM) MJ 1.02E+01 0 0 ­6.05E+00 0 0
Total use of non renewable primary energy resources (PENRT) MJ 2.94E+02 0 2.68E­01 ­6.05E+00 2.38E­01 ­1.27E+02
Use of secondary material (SM) kg 6.06E­01 0 0 0 0 7.66E+00
Use of renewable secondary fuels (RSF) MJ 0 0 0 0 0 0
Use of non renewable secondary fuels (NRSF) MJ 0 0 0 0 0 0
Use of net fresh water (FW) m3 2.78E­01 0 1.76E­05 0 2.46E­06 ­8.28E­01
RESULTS OF THE LCA – WASTE CATEGORIES AND OUTPUT FLOWS according to EN 15804+A2:
1 m² ceiling membrane (0.7 mm; 6.70 kg/m²)
Parameter Unit A1-A3 C1 C2 C3 C4 D
Hazardous waste disposed (HWD) kg 2.16E­07 0 1.41E­11 0 4.22E­11 2.79E­08
Non hazardous waste disposed (NHWD) kg 8.28E­01 0 4.2E­05 0 3.35E­01 1.62E+00
Radioactive waste disposed (RWD) kg 1.24E­03 0 4.86E­07 0 2.72E­06 1.38E­05
Components for re­use (CRU) kg 0 0 0 0 0 0
Materials for recycling (MFR) kg 0 0 0 6.37E+00 0 0
Materials for energy recovery (MER) kg 0 0 0 0 0 0
Exported electrical energy (EEE) MJ 0 0 0 0 0 0
Exported thermal energy (EET) MJ 0 0 0 0 0 0
RESULTS OF THE LCA – additional impact categories according to EN 15804+A2-optional:
1 m² ceiling membrane (0.7 mm; 6.70 kg/m²)
5 Environmental Product Declaration ­ Knauf Ceiling Solutions GmbH & Co. KG ­ Metal Ceiling Membranes (0.7 mm, without acoustic infill)
Parameter Unit A1-A3 C1 C2 C3 C4 D
Disease
Incidence of disease due to PM emissions (PM) 8.03E­07 0 3.77E­10 0 5.65E­10 ­4.4E­07
incidence
Human exposure efficiency relative to U235 (IR) kBq U235 eq 3.85E­01 0 7.1E­05 0 3.89E­04 2.4E­01
Comparative toxic unit for ecosystems (ETP­fw) CTUe 5.59E+01 0 1.98E­01 0 7.01E­02 ­8.23E+00
Comparative toxic unit for humans (carcinogenic) (HTP­c) CTUh 1.19E­08 0 4E­12 0 8.13E­12 ­7.06E­09
Comparative toxic unit for humans (noncarcinogenic) (HTP­nc) CTUh 3.73E­07 0 2.35E­10 0 8.18E­10 ­1.57E­07
Soil quality index (SQP) SQP 5.16E+01 0 9.17E­02 0 1.75E­02 1.91E+00
Disclaimer 1 – for the indicator “Potential Human exposure efficiency relative to U235”. This impact category deals mainly with the
eventual impact of low­dose ionizing radiation on human health of the nuclear fuel cycle. It does not consider effects due to possible
nuclear accidents, occupational exposure or radioactive waste disposal in underground facilities. Potential ionizing radiation from the
soil, radon and from some construction materials is also not measured by this indicator.
Disclaimer 2 – for the indicators “abiotic depletion potential for non­fossil resources”, “abiotic depletion potential for fossil resources”,
“water (user) deprivation potential, deprivation­weighted water consumption”, “potential comparative toxic unit for ecosystems”,
“potential comparative toxic unit for humans – cancerogenic”, “Potential comparative toxic unit for humans ­ not cancerogenic”,
“potential soil quality index”. The results of this environmental impact indicator shall be used with care as the uncertainties on these
results are high as there is limited experience with the indicator.
6. LCA: Interpretation
The following interpretation contains a summary of the LCA weight of 6.70 kg/m² without acoustic infill.
results referenced to a declared unit of 1 m² of average steel
ceiling membrane with a thickness of 0.7 mm and a surface
The comparison of the products' life cycle phases shows a categories considered.
clear dominance of the production phase (modules A1­A3).
Knauf Ceiling Solutions metal ceiling membranes can be
Module C4 declares impacts from landfilling of steel losses specifically configurated based on the customer's need
(assumption: 5 % of steel in the product) making up a minor resulting in more than 100 standard products. The conversion
fraction of the total environmental impact of the products. of the LCA results to other material thicknesses than the
declared reference thickness is proportional to the surface
As a result of material recyclability, the steel fraction removed at weight. As a result, the variability of the environmental impacts
the end of life can substitute primary steel. Module D shows the of single products shows a direct correlation to the product
recycling potential of 95 % of the steel in the product at the end weight.
of its life. This results in credits from the substitution of primary
steel. The declared environmental impacts represent a weighted
average for specific thicknesses of metal ceiling membranes
When it comes to the environmental impacts in the production produced by Knauf Ceiling Solutions considering a
phase of the ceiling membranes, the upstream supply chain of representative perforation of 20 %. It is based on primary data
the steel coils represents the major hot spot in all of the impact of the two production sites of Knauf Ceiling Solutions located at
6 Environmental Product Declaration ­ Knauf Ceiling Solutions GmbH & Co. KG ­ Metal Ceiling Membranes (0.7 mm, without acoustic infill)
Rankweil (AT) and Stafford (UK). identified in all of the impact categories except for potential
ozone depletion and water scarcity.
Comparably higher environmental impacts at Rankweil can be
7. Requisite evidence
The relevant paragraph of the suspended ceiling product containing compound is used during the manufacturing
standard (EN 13964) requires formaldehyde emissions process. Metal ceilings covered by this EPD do not contain any
declaration only for products for which a formaldehyde­ formaldehyde­containing compounds.
8. References
Standards cycle assessment – Requirements and guidelines.
EN 13501-1 Further References
EN 13501­1:2019, Classification of construction products and
building elements according to their reaction to fire, Part 1: AVV
Classification with the results of tests on the reaction to fire of AVV, German List of Wastes Ordinance. Regulation on the
construction products. European Waste List.
EN 13964 Candidate list
EN 13964:2014, Suspended ceilings ­ Requirements and test List of substances of very high concern (SVHC) for
methods. authorisation (ECHA Candidate List), 25.06.2020, published
under Article 59(10) of REACH. Helsinki:
EN 15804 European Chemicals Agency.
EN 15804:2012+A2:2019, Sustainability of construction works ­
Environmental product declarations ­ Core rules for the product European Waste Catalogue
category of construction products. Guidance on classification of waste according to EWC­Stat
categories. Supplement to the Manual for the Implementation of
EN 20140-9 the Regulation (EC) No 2150/2002 on Waste Statistics.
EN ISO 20140­9:1993, Acoustics – Measurement of sound Commission of the European Communities, EUROSTAT.
insulation in buildings.
GaBi
ISO 140-3 GaBi 10, Software­System and Database for Life Cycle
EN ISO 140­3:1995, Acoustics – Measurement of sound Engineering. DB 2021.2. Stuttgart, Echterdingen: Sphera,
insulation in buildings. 1992­2021. Available at:
http://documentation.gabi­software.com
ISO 354
EN ISO 354:2003­12, Acoustics ­ Measurement of sound IBU 2021
absorption in reverberant rooms. Institut Bauen und Umwelt e.V.: Allgemeine Anleitung für das
EPD­­Programm des Institut Bauen und Umwelt e.V. (IBU).
ISO 9001 Version 2.0, Berlin: Institut Bauen und Umwelt e.V., 2021.
EN ISO 9001:2015­11, Quality management systems ­ www.ibu­epd.com
Requirements.
Ordinance on Biocide Products
ISO 11654 Regulation (EU) No 528/2012 of the European Parliament and
EN ISO 11654:1997­07, Acoustics ­ Sound absorbers for use in of the Council of 22 May 2012 concerning the making available
buildings ­ Evaluation of sound absorption. on the market and use of biocidal products.
ISO 14001 PCR part A
EN ISO 14001:2015­11, Environmental management systems ­ Product category rules for building­­related products and
Requirements with guidance for use. services. Part A: Calculation Rules for the Life Cycle
Assessment and Requirements on the Project Report according
ISO 14025 to EN 15804+A2:2019. Version 1.1. Berlin: Institut Bauen und
DIN EN ISO 14025:2011­10, Environmental labels and Umwelt e.V., 2021.
declarations ­ Type III environmental declarations ­ Principles
and procedures. PCR: Metal ceilings
Product category rules for building­related products and
ISO 14044 services. Part B: EPD requirements for metal ceilings. Version
EN ISO 14044:2006­10, Environmental management – Life 1.7. Berlin: Institut Bauen und Umwelt e.V., 08.01.2019.
7 Environmental Product Declaration ­ Knauf Ceiling Solutions GmbH & Co. KG ­ Metal Ceiling Membranes (0.7 mm, without acoustic infill)
Publisher
Institut Bauen und Umwelt e.V. +49 (0)30 3087748­ 0
Hegelplatz 1 info@ibu­epd.com
10117 Berlin www.ibu­epd.com
Germany
Programme holder
Institut Bauen und Umwelt e.V. +49 (0)30 3087748­ 0
Hegelplatz 1 info@ibu­epd.com
10117 Berlin www.ibu­epd.com
Germany
Author of the Life Cycle Assessment
Daxner & Merl GmbH +43 676 849477826
Lindengasse 39/8 office@daxner­merl.com
1070 Wien www.daxner­merl.com
Austria
Owner of the Declaration
Knauf Ceiling Solutions GmbH & Co. KG 0049 8552 422 0
Elsenthal 15 ceiling.solutions@knauf.com
94481 Grafenau www.knaufceilingsolutions.com
Germany
8 Environmental Product Declaration ­ Knauf Ceiling Solutions GmbH & Co. KG ­ Metal Ceiling Membranes (0.7 mm, without acoustic infill)
