ENVIRONMENTAL PRODUCT DECLARATION
as per ISO 14025 and EN 15804+A2
Owner of the Declaration Rubner Holding AG - S.p.A.
Publisher Institut Bauen und Umwelt e.V. (IBU)
Programme holder Institut Bauen und Umwelt e.V. (IBU)
Declaration number EPD-RUB-20230229-IBC1-EN
Issue date 27.06.2023
Valid to 26.06.2028
Structural finger jointed solid timber
Rubner Holding AG - S.p.A
www.ibu-epd.com | https://epd-online.com
1. General Information
Rubner Holding AG - S.p.A Structural finger jointed solid timber
Programme holder Owner of the declaration
IBU – Institut Bauen und Umwelt e.V. Rubner Holding AG - S.p.A.
Hegelplatz 1 Handwerkerzone 2
10117 Berlin 39030 Kiens
Germany Italy
Declaration number Declared product / declared unit
EPD-RUB-20230229-IBC1-EN 1 m³ of solid structural timber [KVH] with an average density of 465 kg/m³
This declaration is based on the product category rules: Scope:
Solid wood products, 01.08.2021 This EPD is based on a declared unit of 1 m³ of solid structural timber
(PCR checked and approved by the SVR) (moisture of 10 % at a raw density of 465 kg/m³) produced at the RUBNER
production site in Ober-Grafendorf (Austria).
Issue date The owner of the declaration shall be liable for the underlying information
and evidence; the IBU shall not be liable with respect to manufacturer
27.06.2023
information, life cycle assessment data and evidences.
The EPD was created according to the specifications of EN 15804+A2. In
Valid to
the following, the standard will be simplified as EN 15804.
26.06.2028
Verification
The standard EN 15804 serves as the core PCR
Independent verification of the declaration and data according to ISO
14025:2011
internally X externally
Dipl.-Ing. Hans Peters
(Chairman of Institut Bauen und Umwelt e.V.)
Florian Pronold Matthias Schulz,
(Managing Director Institut Bauen und Umwelt e.V.) (Independent verifier)
1 Environmental Product Declaration - Rubner Holding AG - S.p.A - Structural finger jointed solid timber
2. Product
Constructional data
2.1 Product description/Product definition
RUBNER structural finger jointed solid timber is a homogenized Name Value Unit
unidirectional wood-based material that is used in engineered Wood types by trade names acc. spruce, pine, larch,
-
structural timber constructions as well as in residential and to EN 1912 Douglas fir
office buildings. RUBNER structural finger jointed solid timber Wood moisture acc. to EN
< 15 %
consists of single squared structured timber made from 13183-1
softwood according to EN 1912. The single structural timber
Use of wood preservatives (the Where other
components with rectangular cross-section are arranged
wood preservative test mark to preservative means -
longitudinally by means of finger joints to achieve a rigid
DIN 68800-3 must be indicated) are insufficient
interconnected structural timber with a rectangular cross-
Bending strength acc. to EN 338 24 N/mm²
section with theoretically infinite length. Due to its longitudinal
assembling characteristics combined with the technically Compressive strength parallel 21 N/mm2
supported strength and stiffness classification of the raw acc. to EN 338
materials, RUBNER structural finger jointed solid timber is Compressive strength
2.5 N/mm2
characterized by a high product quality. As a result of the rectangular acc. to EN 338
industrial manufacturing process, RUBNER structural finger Tensile strength parallel acc. to
14.5 N/mm2
jointed solid timber exhibits steady mechanical characteristics. EN 338
RUBNER structural finger jointed solid timber has a high Tensile strength rectangular acc.
dimensional stability and can be characterized as a largely to EN 338 0.4 N/mm2
crack-minimized building material.
Modulus of elasticity acc. to EN
11000 N/mm2
338
For the placing on the market of the product in the European
Union/European Free Trade Association (EU/EFTA) (with the Shear strength acc. to EN 338 4 N/mm2
exception of Switzerland) Regulation (EU) No. 305/2011 PCR Shear modulus acc. to EN 338 690 N/mm2
applies. The product meets the requirements of EN 15497 and depending on
the CE-marking. Dimensional deviation geometrical mm
For the application and use, the respective national provisions dimensions
apply.
Length < 50 m
2.2 Application Width (min. - max.) 0.06 to 0.28 m
RUBNER structural finger jointed solid timber is mainly used as Height (min. - max.) 0.06 to 0.28 m
a structural component for buildings and bridges. Gross density acc. to EN 338 420 kg/m3
2.3 Technical Data Surface quality (Possible
characteristic features must be n.r. -
The performance data of the product are in accordance with its
indicated)
essential characteristics according to EN 15497.
RUBNER structural finger jointed solid timber is produced in Risk class acc. to DIN 68800-3 4 -
accordance with EN 15497 with different strength classes. For Thermal conductivity acc. to EN
0.12 W/(mK)
the strength class C24, which is mainly used the following 12664
applies: Specific heat capacity acc. to EN
1.6 kJ/kgK
12664
Calculation value for thermal
n.r. W/(mK)
conductivity
Water vapor diffusion equivalent
air layer thickness acc. to ISO n.r. m
12572
Water vapour diffusion resistance
20-50 -
factor acc. to ISO 12572
Formaldehyde emissions acc. to
< E1 μg/m3
EN 15497
RUBNER structural finger jointed solid timber is manufactured
in accordance with EN 15497 from coniferous species, with
priority being given to spruce. Other coniferous species are
permissible but not typical.
RUBNER structural finger jointed solid timber is produced from
kiln-dried coniferous wood with an average wood moisture
content of around 10 % to 11 % (max. < 15 %) at delivery.
For bonding, only approved modern low-emission adhesives
according to chapter 2.5 are used. The mechanical
characteristics of RUBNER structural finger jointed solid timber
are in accordance with strength classes specified in EN 338.
The dimensional tolerances are defined in accordance with EN
15497.
The products are manufactured in domestic visual quality,
visual quality or industrial quality.
2 Environmental Product Declaration - Rubner Holding AG - S.p.A - Structural finger jointed solid timber
Use of preventive chemical wood preservatives in accordance measures and comply with the legal requirements.
with DIN 68800-3 is unusual and permitted only if other The production facility has a quality management system ISO
preservative measures given in DIN 68800-2 are not sufficient 9001.
on their own. The employee protection in the manufacturing process
complies with the respective country-specific requirements,
2.4 Delivery status employees are provided with personal protective equipment.
RUBNER structural finger jointed solid timber is produced with
the dimensions according to chapter 2.3 and is delivered in 2.8 Product processing/Installation
domestic visual quality, visual quality or industrial quality. The RUBNER structural finger jointed solid timber can be processed
tolerances according to EN 15497 are met. with commercially available tools. The instructions for
occupational safety/assembly are to be observed.
2.5 Base materials/Ancillary materials
RUBNER structural finger jointed solid timber comprises kiln- 2.9 Packaging
dried coniferous structural timber with rectangular cross-section Polyethylene foils are used in small quantities during
according to hEN 14081. transportation.
The following types of adhesive systems are used for bonding 2.10 Condition of use
the individual components (finger jointing): The composition of RUBNER structural finger jointed solid
timber corresponds to the composition according to Section 2.5
• Melamine-urea-formaldehyde adhesives (MUF)
for the entire period of use.
RUBNER structural finger jointed solid timber contains the 2.11 Environment and health during use
following proportions of ingredients per m³ on average:
Environmental protection: According to current knowledge, the
• Coniferous wood (atro), mainly spruce approx. 90 % intended use of RUBNER structural finger jointed solid timber
• Water approx. 9-10 % does not present any hazards or impairments to water, air and
• Adhesive < 0.5 % soil.
Health protection: Under normal conditions of use, RUBNER
The product has an average density of 465 kg/m³. structural finger jointed solid timber is not expected to cause
any damage or impairments to health.
This product/article/at least one partial article contains RUBNER structural finger jointed solid timber subsequently
substances listed in the candidate list (date: 17.01.2023) releases formaldehyde during its life cycle.
exceeding 0.1 percentage by mass: no. RUBNER structural finger jointed solid timber bonded with
MUF-based adhesives has low emissions of formaldehyde, due
This product/article/at least one partial article contains other to the low level of adhesive in its internal structure and due to
carcinogenic, mutagenic, reprotoxic (CMR) substances in its particular use. Measured against the limit value of 0.1 ml/m³
categories 1A or 1B which are not on the candidate list, (0.124 mg/m³) of the Reach Regulation 1907/2006/EC, the
exceeding 0.1 percentage by mass: no. measured values in accordance with EN 717-1 can be
classified as low.
Biocide products were added to this construction product or it RUBNER structural finger jointed solid timber with melamine-
has been treated with biocide products (this then concerns a based adhesive system (MUF) has surface-specific emission
treated product as defined by the (EU) Ordinance on Biocide rates in the range of untreated timber.
Products No. 528/2012): no.
2.12 Reference service life
2.6 Manufacture The production processes for RUBNER structural finger jointed
RUBNER structural finger jointed solid timber is manufactured solid timber correspond to the processes that are also used in
from sustainable sawn timber (PEFC, FSC) sourcing from the production laminations for RUBNER glued laminated timber.
sustainable forestry. Wet sawn timber is kiln dried to a moisture Glulam has been used in structural timber construction for more
content of about 10 % (max < 15 %) and subsequently pre- than 100 years. When used as designated, no end of durability
planed. To ensure the characteristic values of the RUBNER must be expected due to its natural durability (protection
structural finger jointed solid timber, all individual structural against moisture). When used as designated, the lifetime of
timber components are visually- or machine-graded regarding RUBNER structural finger jointed solid timber is equal to the
strength and stiffness. Weak parts of components, which duration of use of the building.
reduce the strength and stiffness properties due to the natural
growth characteristics of wood, are cut out depending on the 2.13 Extraordinary effects
grading class. The graded pieces are subsequently bonded by Fire
finger jointing to endless laminations. These laminations with RUBNER structural finger jointed solid timber is classified in
infinite length and a cross section up to 60 * 280 mm² are accordance with EN 15497 as follows:
subsequently planed and cut to the required length for further Fire protection
production. The blanks are planed to achieve the final cross
Name Value
section. If necessary, the blanks are cut to their final complex
Building material class D
shapes. To ensure the product quality, a treatment with
weathering or wood preservatives may be required for transport Burning droplets d0
to the construction site, storage, and during assembly. Smoke gas development s2
2.7 Environment and health during manufacturing
Water
During production, there are no negative impacts on water and
No ingredients are washed out which could be hazardous to
soil. The resulting process wastewater is fed into the local
water.
sewage system and cleaned according to legal regulations. The
resulting exhaust air is cleaned according to the legal
Mechanical destruction
regulations.
The fracture behavior of RUBNER structural finger jointed solid
Noise emissions from industrial plants are reduced by structural
3 Environmental Product Declaration - Rubner Holding AG - S.p.A - Structural finger jointed solid timber
timber is appearance typical for solid wood.
2.15 Disposal
2.14 Re-use phase If the residues are not used for any other cascading use, waste
In the event of selective de-construction, RUBNER structural wood is disposed according to the applicable country-specific
finger jointed solid timber can easily be re-used after the end of requirements. Disposal represents a possible but unusual case.
the structure's service life. RUBNER structural finger jointed solid timber is assigned to
The preferred use of RUBNER structural finger jointed solid waste code 17 02 01 in the European list of waste
timber is in the form of reuse based on the applicable country- 2014/955/EU. (Treated Rubner structural finger jointed solid
specific requirements. timber is assigned to waste code 17 02 04).
If it is not re-used, it will be subjected to thermal utilization for
the production of heat and electricity due to the high calorific 2.16 Further information
value of approx. 16.5 MJ/kg (at a humidity of u = 12 %) in More detailed information is available at: www.rubner.com
compliance with the applicable country-specific requirements.
3. LCA: Calculation rules
Module C1 | Deconstruction and demolition
3.1 Declared Unit After the removal of building components overlying the product,
This EPD refers to a declared unit of 1 m³ of solid structural the joints can simply be loosened by screwing or sawing and
timber produced by the RUBNER group. The declared unit lifted by cranes to the place of removal. Required energy
refers to an average density of 465 kg/m³ and a wood moisture demand can be neglected. The actual energy demand depends
at delivery of 10 %. on the installation of the products and can therefore vary
Declared unit greatly in the building context.
Name Value Unit
Module C2 | Transport to disposal
Declared unit 1 m3 Module C2 includes the transport to waste treatment. In this
Gross density 465 kg/m3 case, transport by truck over a transport distance of 50 km is
Wood moisture at delivery 10 % assumed.
The analysed products represent an average of RUBNER solid
Module C3 | Waste processing
structural timber produced at the site in Ober-Grafendorf (AT).
In Module C3, the chipping after the removal of the products is
considered. The wooden products and with them the material-
The declared unit was calculated on a volume-weighted basis.
inherent properties leave the product system as secondary
This EPD refers to an average product manufactured at one
combustibles in module C3.
site. All products undergo the same processing steps. A
possible variability is only expected due to the use of different
Module C4 | Disposal
wood species. The upstream chain for spruce is considered
The applied scenario declares the energetic recovery of the
representative. The robustness of the declared LCA values can
wooden products, therefore no environmental impacts are to be
thus be classified as high.
expected from waste processing of the products in C4.
Ober-Grafendorf not only produces solid structural timber but
Module D | Benefits and loads beyond the system
also glued laminated timber. The allocation of product-specific
boundary
material and energy flows is based on physical relationships
Applying an European average scenario, module D describes
when possible. Where necessary, the allocation is based on the
the energetic recovery of the product at the end of life including
production volumes of each product line manufactured at Ober-
the corresponding energy substitution potentials.
Grafendorf.
3.3 Estimates and assumptions
3.2 System boundary
All assumptions are verified through detailed documentation
The life cycle assessment of average solid structural timber
and correspond to the best possible representation of reality
produced by RUBNER refers to a cradle-to-gate analysis of the
based on the available data. Background data for wood logs
environmental impacts with modules C1–C4 and module D
refer to generic data for spruce logs in bark derived from GaBi
(A1–A3 + C + D). The following life cycle phases are part of the
database. Spruce represents the majority of wood processed at
analysis:
RUBNER. The used dataset represents an approximation for all
other species.
Module A1–A3 | Production stage
Regional applicability of the used background data refers to
The production stage includes the upstream burdens of raw
average data under European or German conditions taken from
materials (lamellae, adhesive system, etc.) and the
the GaBi database. German data were used for the Austrian
corresponding transports to the RUBNER production site in
market whenever European or regionalised average data were
Ober-Grafendorf (Austria). As the production site in Rohrbach
not available.
delivers lamellae to the other RUBNER sites, resulting
environmental impacts refer to RUBNER's specific production
Emissions from wood drying were included in the calculations
process including drying. Direct emissions from drying are
according to Rüter & Diederichs 2012.
based on worst-case approximations and are included in the
study. Upstream emissions from the use of adhesive systems 3.4 Cut-off criteria
rely on supplier-specific data. The LCA model covers all available input and output flows,
RUBNER produces thermal energy in its own biomass boilers. which can be represented based on robust data and from which
Electricity is provided by the own photovoltaic system as well as a significant contribution can be expected. Data gaps are filled
100 % green electricity. with conservative assumptions of average data or generic data
if available and are documented accordingly.
Only data with a contribution of less than 1 % were cut off.
4 Environmental Product Declaration - Rubner Holding AG - S.p.A - Structural finger jointed solid timber
Thus, no data were neglected, of which a substantial impact is high data quality.
to be expected. All relevant data were collected The technological, geographical and time-related
comprehensively. Cutoff material and energy flows were representativeness of the database was kept in mind when
chosen carefully based on their expected quantitative selecting background data. Whenever specific data were
contribution as well as potential environmental impacts. Thus, it missing, either generic datasets or representative average data
can be assumed that the sum of all neglected input flows does were used instead. The implemented GaBi background
not account for more than 5 % of the total material, water and datasets refer to the latest versions available and are carefully
energy flows. Environmental impacts of machines, plant and chosen.
infrastructure were not included.
The assessment of the robustness of the average can be found
3.5 Background data in Section 3.1.
This study uses generic background data for the evaluation of
upstream environmental impacts from GaBi database 2022.2 3.7 Period under review
as well as recognised literature such as Rüter & Diederichs Foreground data were collected in the 2022 production year,
2012. and the data are based on the volumes produced on an annual
basis.
The main share of lamellae processed for solid structural timber
is delivered by the RUBNER RHI located in Rohrbach. Thus, 3.8 Geographic Representativeness
the supply chain for lamellae input is based on primary data. Land or region, in which the declared product system is
The representation of adhesives used for the production is manufactured, used or handled at the end of the product´s
based on primary data from RUBNER's suppliers. Where lifespan: Austria
necessary, this information was complemented with estimates
ensuring the completeness of the component's representation
3.9 Allocation
in the LCA.
Carbon content and primary energy content of the products
3.6 Data quality were assessed based on their material
Data collection is based on product-specific questionnaires. It inherent properties according to underlying physical
follows an iterative process of clarifying questions via e-mail, relationships.
telephone calls or in personal/web meetings. Intensive
3.10 Comparability
discussions between the RUBNER group and Daxner & Merl
Basically, a comparison or an evaluation of EPD data is only
result in an accurate mapping of product-related material and
possible if all the data sets to be compared were created
energy flows. This leads to a high quality of foreground data
according to EN 15804 and the building context, respectively
collected. Data collection relies on a consistent process
the product-specific characteristics of performance, are taken
according to ISO 14044.
into account.
The representation of the main raw materials used for the
The GaBi background database was used to calculate the LCA
production of solid structural timber is based on supplier-
(GaBi 10; 2022.2).
specific primary data (lamellae, adhesive systems) leading to a
4. LCA: Scenarios and additional technical information
End of life (C1-C4)
Characteristic product properties of biogenic carbon
During tree growth, the wood assimilates carbon dioxide and Name Value Unit
stores biogenic carbon. The carbon stored in the product is Energy recovery 465 kg
declared in the following table.
Reuse, recovery and/or recycling potentials (D), relevant
Information on describing the biogenic Carbon Content at
scenario information
factory gate
Name Value Unit
Name Value Unit
Processing rate 100 %
Biogenic carbon content in product 211 kg C
Efficiency of power plant 68 %
The product reaches the end-of-waste status after removal from
the building, transport to processing and chipping of the
product. For the end of life of the solid structural timber product,
Installation into the building (A5) energy recovery as secondary fuel in a biomass power plant is
The end of life of the product packaging is not declared in assumed. As the main sales market for the solid wood products
module A5. is concentrated in the European region, plant-specific
Name Value Unit characteristic values correspond to a European average
scenario (EU). The scenario considers a reprocessing rate of
Packaging (polyethylene) 0.409 kg
100 % for the solid wood products after removal from the
building. This assumption has to be adjusted accordingly when
The end-of-life scenario used in this LCA study is based on the applying the results in the building context. At the end of life of
following assumptions: the product, the equilibrium moisture is comparable to the
moisture content at delivery. This value can vary depending on
the storage of the product before energy recovery.
5 Environmental Product Declaration - Rubner Holding AG - S.p.A - Structural finger jointed solid timber
5. LCA: Results
The following table contains the LCA results for a declared unit of 1 m³ of solid structural timber produced by the RUBNER group
(465 kg/m³).
DESCRIPTION OF THE SYSTEM BOUNDARY (X = INCLUDED IN LCA; ND = MODULE OR INDICATOR NOT DECLARED; MNR =
MODULE NOT RELEVANT)
Benefits and
Construction loads beyond
Product stage Use stage End-of-life stage
process stage the system
boundaries
la ire ta m w a Ry lp p u s tro p s n a rT g n iru tc a fu n a M e h t m o rf tro p s n a rTe tis e h t o t e ta g y lb m e s s A e s U e c n a n e tn ia M ria p e R tn e m e c a lp e R tn e m h s ib ru fe R y g re n e la n o ita re p Oe s u re ta w la n o ita re p Oe s u n o itc u rts n o c -e Dn o itilo m e d tro p s n a rT g n is s e c o rp e ts a W la s o p s iD -e s u e R-y re v o c e R-g n ilc y c e Rla itn e to p
A1 A2 A3 A4 A5 B1 B2 B3 B4 B5 B6 B7 C1 C2 C3 C4 D
X X X MND MND MND MND MNR MNR MNR MND MND X X X X X
RESULTS OF THE LCA - ENVIRONMENTAL IMPACT according to EN 15804+A2: 1 m³ solid structural timber (465 kg/m³)
Parameter Unit A1-A3 C1 C2 C3 C4 D
Global Warming Potential total (GWP-total) kg CO 2 eq -7.07E+02 0 1.47E+00 7.84E+02 0 -4.28E+02
Global Warming Potential fossil fuels (GWP-fossil) kg CO 2 eq 6.71E+01 0 1.4E+00 3.43E+00 0 -3.86E+02
Global Warming Potential biogenic (GWP-biogenic) kg CO 2 eq -7.75E+02 0 6.1E-02 7.8E+02 0 -4.18E+01
Global Warming Potential luluc (GWP-luluc) kg CO 2 eq 3.17E-01 0 9.41E-03 7.25E-04 0 -4.62E-02
Depletion potential of the stratospheric ozone layer (ODP) kg CFC11 eq 2.82E-09 0 1.37E-13 5.02E-11 0 -2.99E-09
Acidification potential of land and water (AP) mol H+ eq 8.26E-01 0 4.66E-03 7.53E-03 0 3.2E-01
Eutrophication potential aquatic freshwater (EP-freshwater) kg P eq 5.42E-03 0 4.99E-06 1E-05 0 -6.03E-04
Eutrophication potential aquatic marine (EP-marine) kg N eq 3.28E-01 0 2.13E-03 1.69E-03 0 6.94E-02
Eutrophication potential terrestrial (EP-terrestrial) mol N eq 2.93E+00 0 2.39E-02 1.77E-02 0 8.22E-01
Formation potential of tropospheric ozone photochemical oxidants kg NMVOC
9.32E-01 0 4.19E-03 4.57E-03 0 2.94E-01
(POCP) eq
Abiotic depletion potential for non fossil resources (ADPE) kg Sb eq 3.96E-05 0 1.41E-07 9.35E-07 0 -6.41E-05
Abiotic depletion potential for fossil resources (ADPF) MJ 8.55E+02 0 1.83E+01 6.23E+01 0 -6.68E+03
m3 world eq
Water use (WDP) 3.4E+01 0 1.56E-02 7.82E-01 0 -2.2E+01
deprived
RESULTS OF THE LCA - INDICATORS TO DESCRIBE RESOURCE USE according to EN 15804+A2: 1 m³ solid structural timber
(465 kg/m³)
Parameter Unit A1-A3 C1 C2 C3 C4 D
Renewable primary energy as energy carrier (PERE) MJ 5.51E+03 0 1.27E+00 7.83E+03 0 -2.06E+03
Renewable primary energy resources as material utilization
MJ 7.8E+03 0 0 -7.8E+03 0 0
(PERM)
Total use of renewable primary energy resources (PERT) MJ 1.33E+04 0 1.27E+00 3.46E+01 0 -2.06E+03
Non renewable primary energy as energy carrier (PENRE) MJ 8.25E+02 0 1.84E+01 7.74E+01 0 -6.68E+03
Non renewable primary energy as material utilization (PENRM) MJ 3.28E+01 0 0 -1.51E+01 0 0
Total use of non renewable primary energy resources (PENRT) MJ 8.58E+02 0 1.84E+01 6.23E+01 0 -6.68E+03
Use of secondary material (SM) kg 0 0 0 0 0 0
Use of renewable secondary fuels (RSF) MJ 0 0 0 0 0 7.8E+03
Use of non renewable secondary fuels (NRSF) MJ 0 0 0 0 0 1.51E+01
Use of net fresh water (FW) m3 1.4E+00 0 1.47E-03 3.3E-02 0 -1.4E+00
RESULTS OF THE LCA – WASTE CATEGORIES AND OUTPUT FLOWS according to EN 15804+A2:
1 m³ solid structural timber (465 kg/m³)
Parameter Unit A1-A3 C1 C2 C3 C4 D
Hazardous waste disposed (HWD) kg 4.71E-07 0 9.73E-11 5.39E-09 0 -8.27E-07
Non hazardous waste disposed (NHWD) kg 4.65E+00 0 3E-03 4.69E-02 0 2.31E-01
Radioactive waste disposed (RWD) kg 1.42E-02 0 3.41E-05 9.95E-03 0 -5.91E-01
Components for re-use (CRU) kg 0 0 0 0 0 0
Materials for recycling (MFR) kg 0 0 0 0 0 0
Materials for energy recovery (MER) kg 0 0 0 4.65E+02 0 0
Exported electrical energy (EEE) MJ 0 0 0 0 0 0
Exported thermal energy (EET) MJ 0 0 0 0 0 0
RESULTS OF THE LCA – additional impact categories according to EN 15804+A2-optional:
1 m³ solid structural timber (465 kg/m³)
Parameter Unit A1-A3 C1 C2 C3 C4 D
Incidence of disease due to PM emissions (PM) Disease ND ND ND ND ND ND
6 Environmental Product Declaration - Rubner Holding AG - S.p.A - Structural finger jointed solid timber
incidence
Human exposure efficiency relative to U235 (IR) kBq U235 eq ND ND ND ND ND ND
Comparative toxic unit for ecosystems (ETP-fw) CTUe ND ND ND ND ND ND
Comparative toxic unit for humans (carcinogenic) (HTP-c) CTUh ND ND ND ND ND ND
Comparative toxic unit for humans (noncarcinogenic) (HTP-nc) CTUh ND ND ND ND ND ND
Soil quality index (SQP) SQP ND ND ND ND ND ND
The additional and optional impact categories according to EN 15804+A2 are not declared, as the uncertainty of these indicators is to
be classified as high.
Disclaimer 1 – for the indicator 'Potential Human exposure efficiency relative to U235'.
This impact category deals mainly with the eventual impact of lowdose ionizing radiation on human health of the nuclear fuel cycle. It
does not consider effects due to possible nuclear accidents, occupational exposure or radioactive waste disposal in underground
facilities. Potential ionizing radiation from the soil, from radon and from some construction materials is also not measured by this
indicator.
Disclaimer 2 – for the indicators 'abiotic depletion potential for non-fossil resources', 'abiotic depletion potential for fossil resources',
'water (user) deprivation potential, deprivation-weighted water consumption', 'potential comparative toxic unit for ecosystems', 'potential
comparative toxic unit for humans – cancerogenic', 'Potential comparative toxic unit for humans - not cancerogenic', 'potential soil
quality index'.
The results of this environmental impact indicator shall be used with care as the uncertainties on these results are high as there is
limited experience with the indicator.
6. LCA: Interpretation
The following interpretation contains a summary of the LCA After its use in the building, the product is assumed to be
results referenced to a declared unit of 1 m³ of solid structural incinerated in a biomass power plant. As a result, the
timber. incorporated carbon is emitted again to the atmosphere
representing biogenic carbon dioxide emissions (module C3).
The global warming potential (GWP) of solid structural timber
shows negative values in the production phase (modules A1– The negative values in the end-of-life (module D) result from
A3). These negative impacts result from the use of wood as raw the energetic treatment of the product. As the energy produced
material. Wood sequesters biogenic carbon during tree growth. at the biomass power plant can substitute (mainly fossil) fuels,
The sequestered carbon does not contribute to global warming an environmental net benefit is generated.
as long as it is stored in the biomass.
Potential global warming (GWP) due to the production of solid carbon neutral, as the wood is derived from sustainably
structural timber mainly stems from the provision of round wood managed forests.
and associated impacts due to forestry. The processing of the
products includes the use of all wooden residues for heat In all environmental impact categories considered (with the
production. Its thermal treatment is taken into account as exception of ODP), the upstream chain of the supplied lamellae
7 Environmental Product Declaration - Rubner Holding AG - S.p.A - Structural finger jointed solid timber
represents the main factor in the LCA. What's more, the factor in the environmental profile of the product.
provision of thermal energy from on-site biomass boilers and
transports are further drivers. The results of the previous EPD (EPD-RUB-20180059-IBB1-
EN) are not directly comparable with the present updated
Due to the use of green electricity in the production, the version due to the update of the underlying methodology
external supply of electricity at the site represents a minor according to EN 15804+A2.
7. Requisite evidence
The following evidence of environmental and health relevance 7.4 VOC emissions
was provided. For the verification of VOC emissions, one test report (51005-
001 III, 2016) of an emission analysis according to AgBB-
7.1 Formaldehyde Scheme 2015 for Rubner glulam is available. Analysis was
The emissions (melamine-based adhesive systems) listed in performed in accordance with ISO 16000-3 and ISO 16000-6.
section 2.11 are based on test results of emission The listed values represent upper limit values due to the
measurements in accordance with EN 717-1 at a temperature significantly lower adhesive content of RUBNER structural
of 23 °C, a relative humidity of 45 % and an air change rate of finger jointed solid timber compared to Rubner glulam.
1.0 per hour. The test results all meet the requirements of RUBNER structural finger jointed solid timber contains less
emission class E1 according to EN 15497 of 0.124 mg/m³. than 0.5 % adhesive. Based on these facts, VOC emissions
The test report (E-CMP / KT T410 405, 2016) defines a from the glue of RUBNER structural finger jointed solid timber is
formaldehyde emission of 0.011 mg/m³ for Rubner glulam made significantly lower. Due to the arbitrary position of the finger
of spruce with melamine-based adhesive. The listed value joints no product representative test specimen can be defined,
represents an upper limit value due to the significantly lower therefore no representative test can be done.
adhesive content, RUBNER structural finger jointed solid timber
VOC emissions
contains only 10 % adhesive compared to Rubner glulam.
Name Value Unit
Based on these facts formaldehyde emission of RUBNER
structural finger jointed solid timber is significantly below 0.01 Overview of Results (28 days) - μg/m3
mg/m³. Due to the arbitrary position of the finger joints, no TVOC (C6 - C16) acc. to AgBB 2015 70 μg/m3
product representative test specimen can be defined, therefore
Sum SVOC (C16 - C22) acc. to AgBB 2015 < 5 μg/m3
no representative test can be done.
R (dimensionless) acc. to AgBB 2015 0.17 -
There is one test report for proof of occupational exposure
(Dräger Kurzzeitröhrchen) (date 16. June 2015) available, the VOC without NIK acc. to AgBB 2015 <5 μg/m3
maximum allowed workplace concentration of 0.246 mg/m³ is Carcinogenic Substances <1 μg/m3
significantly higher than the measurements, no discolouration
For the verification of VOC emissions, one test report (51005-
of the tubes was noted.
002 III B, 2016) of an emission analysis according to AgBB-
Scheme 2015 for pure wood is available. Analysis was
7.2 MDI
performed in accordance with ISO 16000-3 and ISO 16000-6.
In the context of production, no such substances are added to
The listed values represent lower limit values.
the wood. Thus, a MDI emission from the finished RUBNER
structural finger jointed solid timber is not possible. VOC emissions: pure wood
Name Value Unit
7.3 Fire gas toxicity
Overview of Results (28 days) - μg/m³
Due to the heterogeneous structure of structural finger jointed
TVOC (C6 - C16) acc. to AgBB 2015 10 μg/m³
solid timber, combined with the non-applicability of the test
standard DIN 53436, no relevant measurement results are Sum SVOC (C16 - C22) acc. to AgBB 2015 <5 μg/m³
available, the test specimen geometry is not able to represent R (dimensionless) acc. to AgBB 2015 0.086 -
the real gas composition for a representative cross-section. VOC without NIK acc. to AgBB 2015 <5 μg/m³
Carcinogenic Substances <1 μg/m³
8. References
Standards EN 717-1
DIN EN 717-1:2005-01, Wood-based panels – Determination of
DIN 53436 Formaldehyde release – Part 1: Formaldehyde emission by the
DIN 53436:2015, Generation of thermal decomposition chamber method.
products from materials for their analytic-toxicological testing.
EN 1912
DIN 68800-2 EN 1912: 2013-10-15, Structural timber - Strength classes -
DIN 68800-2:2012-02, Wood preservation – Part 2: Preventive Assignment of visual grades and species.
constructional measures in buildings.
EN 12664
DIN 68800-3 EN 12664:2001, Thermal performance of building materials and
DIN 68800-3:2012-02, Wood preservation – Part 3: Preventive products - Determination of thermal resistance by means of
protection of wood with wood preservatives. guarded hot plate and heat flow meter methods - Dry and moist
products with medium and low thermal resistance.
EN 338
DIN EN 338:2016-07, Structural timber - Strength classes. EN 13183-1
EN 13183-1:2002, Moisture content of a piece of sawn.
8 Environmental Product Declaration - Rubner Holding AG - S.p.A - Structural finger jointed solid timber
EN 15497 (status 17.01.2023) according to Article 59 para. 10 of the
DIN EN 15497:2014-07, Structural finger jointed solid timber - REACH Regulation. European Chemicals Agency.
Performance requirements and minimum production
requirements. GaBi
GaBi 10, Software-System and Database for Life Cycle
EN 15804 Engineering. 2022.2. Stuttgart, Echterdingen: Sphera, 1992-
DIN EN 15804:2012+A2:2019+AC:2021, Sustainability of 2022. Available at: https://sphera.com/product-sustainability-
construction works Environmental product declarations Core gabi-data-search/
rules for the product category of construction products.
IBU 2021
hEN 14081 Institut Bauen und Umwelt e.V.: General Programme
hEN 14081-1:2016-06-01, Timber structures - Strength graded Instructions for the Preparation of EPDs at the Institut Bauen
structural timber with rectangular cross section - Part 1: und Umwelt e.V. (IBU). Version 2.0, Berlin: Institut Bauen und
General requirements. Umwelt e.V., 2021. www.ibuepd.com
ISO 9001 Ordinance on Biocide Products
EN ISO 9001:2015, Quality management systems - Regulation (EU) No 528/2012 of the European Parliament and
Requirements. of the Council of 22 May 2012 concerning the making available
on the market and use of biocidal products.
ISO 12572
EN ISO 12572:2016, Hygrothermal performance of building PCR part A
materials and products - Determination of water vapour Product category rules for building-related products and
transmission properties - Cup method. services. Part A: Calculation Rules for the Life Cycle
Assessment and Requirements on the Project Report according
ISO 14025 to EN 15804+A2:2019. Version 1.3. Berlin: Institut Bauen und
DIN EN ISO 14025:2011-10, Environmental labels and Umwelt e.V., 2022.
declarations Type III environmental declarations Principles and
procedures. PCR: Solid wood products
Product category rules for building-related products and
ISO 14044 services. Part B: EPD requirements for solid wood products.
DIN EN ISO 14044:2006-10, Environmental management - Life Version v2, Berlin: Institut Bauen und Umwelt e.V., 31.05.2023.
cycle assessment - Requirements and guidelines.
PCR 305/2011 (EU)
ISO 16000-3 REGULATION (EU) No 305/2011 OF THE EUROPEAN
ISO 16000-3:2011 Indoor air - Part 3: Determination of PARLIAMENT AND OF THE COUNCIL of 9 March 2011 laying
formaldehyde and other carbonyl compounds in indoor air and down harmonised conditions for the marketing of construction
test chamber air - Active sampling method. products and repealing Council Directive 89/106/EEC.
ISO 16000-6 Rüter & Diederichs 2012
ISO 16000-6:2011 Indoor air - Part 6: Determination of volatile Ökobilanz-Basisdaten für Bauprodukte aus Holz. Work report
organic compounds in indoor and test chamber air by active from the Institut für Holztechnologie und Holzbiologie Nr.
sampling on Tenax TA® sorbent, thermal desorption and gas 2012/1. Hamburg: Johann Heinrich von Thünen-Institut.
chromatography using MS or MS-FID.
1907/2006/EG
VERORDNUNG (EG) Nr. 1907/2006 DES EUROPÄISCHEN
Further references PARLAMENTS UND DES RATES vom 18. Dezember 2006 zur
Registrierung, Bewertung, Zulassung und Beschränkung
AgBB-Scheme 2015 chemischer Stoffe (REACH).
German Committee for HealthRelated Evaluation of Building
Products (AgBB): Approach to health assessment of emissions 2014/955/EU
of volatile organic compounds (VOCs and SVOCs) from 2014/955/EU,COMMISSION DECISION of 18 December 2014
building products. amending Decision 2000/532/EC on the list of waste pursuant
to Directive 2008/98/EC of the European Parliament and of the
Candidate List Council.
List of substances of very high concern considered for approval
9 Environmental Product Declaration - Rubner Holding AG - S.p.A - Structural finger jointed solid timber
Publisher
Institut Bauen und Umwelt e.V. +49 (0)30 3087748- 0
Hegelplatz 1 info@ibu-epd.com
10117 Berlin www.ibu-epd.com
Germany
Programme holder
Institut Bauen und Umwelt e.V. +49 (0)30 3087748- 0
Hegelplatz 1 info@ibu-epd.com
10117 Berlin www.ibu-epd.com
Germany
Author of the Life Cycle Assessment
Daxner & Merl GmbH +43 676 849477826
Schleifmühlgasse 13/24 office@daxner-merl.com
1040 Wien www.daxner-merl.com
Austria
Owner of the Declaration
Rubner Holding AG - S.p.A. 0039 0474 563 777
Handwerkerzone 2 info@rubner.com
39030 Kiens www.rubner.com
Italy
10 Environmental Product Declaration - Rubner Holding AG - S.p.A - Structural finger jointed solid timber
