ENVIRONMENTAL PRODUCT DECLARATION
as per ISO 14025 and EN 15804+A2
Owner of the Declaration dormakaba International Holding GmbH
Publisher Institut Bauen und Umwelt e.V. (IBU)
Programme holder Institut Bauen und Umwelt e.V. (IBU)
Declaration number EPD-DOR-20230214-CBA1-EN
Issue date 21.08.2023
Valid to 20.08.2028
Automatic revolving door KTC 2
dormakaba
www.ibu-epd.com | https://epd-online.com
General Information
dormakaba Automatic revolving door KTC 2
Programme holder Owner of the declaration
IBU – Institut Bauen und Umwelt e.V. dormakaba International Holding GmbH
Hegelplatz 1 DORMA Platz 1
10117 Berlin 58256 Ennepetal
Germany Germany
Declaration number Declared product / declared unit
EPD-DOR-20230214-CBA1-EN 1 piece of the product: Automatic Revolving Door KTC 2 diameter 4,8m
and clear passage height 2,4m, consisting of the following items:
• Two wings
• Integrated sliding door
• Automatic sliding door operator
• Canopy
• Showcases
• Drum walls
• Product packaging
This declaration is based on the product category rules: Scope:
Automatic doors, automatic gates, and revolving door systems, This Environmental Product Declaration refers to a specific revolving door
01.08.2021 manufactured by dormakaba.The production site is located in Suzhou
(PCR checked and approved by the SVR) (China).
The data represent the year 2022.
Issue date
The owner of the declaration shall be liable for the underlying information
21.08.2023
and evidence; the IBU shall not be liable with respect to manufacturer
information, life cycle assessment data and evidences.
Valid to
The EPD was created according to the specifications of EN 15804+A2. In
20.08.2028 the following, the standard will be simplified as EN 15804.
Verification
The standard EN 15804 serves as the core PCR
Independent verification of the declaration and data according to ISO
14025:2011
internally X externally
Dipl.-Ing. Hans Peters
(Chairman of Institut Bauen und Umwelt e.V.)
Florian Pronold Dr.-Ing. Wolfram Trinius,
(Managing Director Institut Bauen und Umwelt e.V.) (Independent verifier)
1 Environmental Product Declaration - dormakaba - Automatic revolving door KTC 2
Product
Product description/Product definition Base materials/Ancillary materials
The automatic revolving door KTC 2 combines extensive The major material composition including the packaging of the
functions, robust technology and attractive design product is listed below:
Name Value Unit
KTC 2 revolving door systems with integrated automatic sliding
Glass 34 %
door offers a wide range of adjustment possibilities. Due to
Aluminium 34 %
changing access requirements of large buildings over the
course of the day and during the evening a versatile door Steel 23 %
system that is quickly adaptable to requirements is the ideal Wood 3 %
solution. Plastic 2 %
Electronic 2 %
KTC 2 high-capacity doors are designed and manufactured to
Paper 2 %
suit individual requirements and are reliable at the same time.
The door systems allows entry in a short period of time and are The product includes partial articles which contain substances
securely looked whenever needed. For the use and application listed in the Candidate List of REACH Regulation
of the product the respective national provisons at the place of 1907/2006/EC (date: 14.06.2023) exceeding 0.1 percentage by
use apply. For the automatic revolving door KTC 2 the mass: yes
standards which can be applied are the following:
• Lead (Pb): 7439-92-1 (CASNo) is included in the battery
• ISO 13849-1
and some of the alloys used. The concentration in each
• ISO 12100
individual alloy does not exceed 4% (by mass).
• DIN 18650-1
• DIN 18650-2
The Candidate List can be found on the ECHA website
• EN 16005
address: https:echa.europa.eu/de/home.
• EN 60335-1
• EN 61000
Reference service life
• 2011/65/EU ROHS3 Directive
The reference service life for the automatic revolving door KTC
• Machinery Directive 2006/42/EC
2 amounts to 20 years and depends on the application and
frequency of use. For repairs and renewals, suitable spare
The CE marking takes into account the proof of conformity with
parts are available. The revolving door is tested and certified to
the respective harmonized standards based on the legal
EN 16005, meaning they are designed to withstand a minimum
provisions above.
of 1.000.000 cycles.
Application
Automatic revolving doors may be used to provide a
comfortable entry and exit in many applications in the facade of
or within a building.
The KTC 2 is ideal for the use in:
• Hotels
• Healthcare settings
• Airports and transportation facilities
• Commercial office buildings
• Institutional and educational buildings
• Retail stores
Technical Data
The automatic revolving door KTC 2 has following technical
properties:
Name Value Unit
Power consumption on mode 184,8 W
Power consumption idle mode 80,8 W
Power consumption off mode 80,8 W
Internal diameter of the drum 3000-5400 mm
Width of the door unit 3210-5610 mm
Performance data of the product with respect to its
characteristics in accordance with the relevant technical
provision which can be applied are mentioned above.
2 Environmental Product Declaration - dormakaba - Automatic revolving door KTC 2
LCA: Calculation rules
Use stage - Module B6
Declared Unit The use stage related to the operation of the building
The declared unit is 1 piece of the product: KTC 2 includes:
Name Value Unit — B6, operational energy use
Declared unit 1 pce.
End-of-life stage– Modules C1-C4 and D
Mass reference of declared product 2445 kg/pce
The end-of-life stage includes:
— C1, deconstruction, demolition:
— C2, transport to waste processing;
System boundary
— C3, waste processing for reuse, recovery and/or
The type of EPD is: cradle to gate with options,
recycling;
modules C1–C4, and module D (A1–A3 + C + D and
— C4, disposal;
additional modules: A4 + A5 + B6)
including provision and all transport, provision of all
materials, products and related energy and water use.
Production - Module A1-A3
Module D (Benefits and loads beyond the system
The product stage includes:
boundary) includes:
— A1, raw material extraction, processing and
— D, recycling potentials, expressed as net impacts
mechanical treatments, processing of secondary
and benefits.
material input (e.g. recycling processes),
— A2, transport to the manufacturer, Geographic Representativeness
— A3, manufacturing and assembly including provision Land or region, in which the declared product system is
of all materials, products and energy, as well as waste manufactured, used or handled at the end of the product´s
processing up to the end-of waste state. lifespan: Global
Construction stage - Modules A4-A5
The construction process stage includes: Comparability
— A4, transport to the building site; Basically, a comparison or an evaluation of EPD data is only
— A5, installation into the building; possible if all the data sets to be compared were created
including provision of all materials, products and according to EN 15804 and the building context, respectively
energy, as well as waste processing up to the end-of the product-specific characteristics of performance, are taken
waste state or disposal of final residues during the into account. Background database: GaBi, SP40
construction process stage.
LCA: Scenarios and additional technical information
Transport to the building site (A4)
Characteristic product properties of biogenic carbon
The following technical scenario information is required for the
The biogenic carbon content quantifies the amount of biogenic
declared modules
carbon in a construction product leaving the factory gate, and it
shall be separately declared for the product and for any Name Value Unit
accompanying packaging. Litres of fuel 0.00276 l/100km
If the total mass of biogenic carbon containing materials is less Capacity utilisation (including empty runs) 55 %
than 5 % of the total mass of the product and accompanying
Transport distance via medium truck 100 km
packaging, the declaration of biogenic carbon content may be
Transport distance via ship 1000 km
omitted. The mass of packaging containing biogenic carbon
shall always be declared. The product is transported via truck and ship. The main
distribution regions are Europe and China. In order to allow
Note: 1 kg of biogenic carbon is equivalent to 44/12 kg of CO2. scaling to a specific point of installation 100 km are declared.
Information on describing the biogenic carbon content at
factury gate Reference service life
Name ValueUnit Name Value Unit
kg Life Span according to the manufacturer 20 a
Biogenic carbon content in product 39.21
C
Biogenic carbon content in accompanying kg
18.41
packaging C
3 Environmental Product Declaration - dormakaba - Automatic revolving door KTC 2
Operational energy use (B6) Reuse, recovery and/or recycling potentials (D), relevant
Name Value Unit scenario information
Electricity consumption for 1 year 935.97 kWh Name Value Unit
Days per year in use 365 days Recycling 100 %
On mode per day 6 h The collection rate is 100%.
Idle mode per day 4 h
Off mode per day 14 h
On mode 184,8 W
Idle mode 80,8 W
Off mode 80,8 W
End of life (C1-C4)
C1: The product expansion depends on the building. The
product share is so low that no environmental burden is
assumed.
C2: Transport to waste management 50 km.
Name Value Unit
Collected separately waste type 2390 kg
Recycling 1430 kg
Energy recovery 44.3 kg
Landfilling 911 kg
The product is disassembled in a recycling process. Material
recycling is then assumed for the metals and electronics. The
plastic components are assumed to be incinerated with energy
recovery. Electromechanics and minor proportions of residues
arising from the recycling process are landfilled. Region for the
End of Life is: Global.
4 Environmental Product Declaration - dormakaba - Automatic revolving door KTC 2
LCA: Results
DESCRIPTION OF THE SYSTEM BOUNDARY (X = INCLUDED IN LCA; ND = MODULE OR INDICATOR NOT DECLARED; MNR =
MODULE NOT RELEVANT)
Benefits and
Construction loads beyond
Product stage Use stage End-of-life stage
process stage the system
boundaries
la ire ta m w a Ry lp p u s tro p s n a rT g n iru tc a fu n a M e h t m o rf tro p s n a rTe tis e h t o t e ta g y lb m e s s A e s U e c n a n e tn ia M ria p e R tn e m e c a lp e R tn e m h s ib ru fe R y g re n e la n o ita re p Oe s u re ta w la n o ita re p Oe s u n o itc u rts n o c -e Dn o itilo m e d tro p s n a rT g n is s e c o rp e ts a W la s o p s iD -e s u e R-y re v o c e R-g n ilc y c e Rla itn e to p
A1 A2 A3 A4 A5 B1 B2 B3 B4 B5 B6 B7 C1 C2 C3 C4 D
X X X X X MND MND MNR MNR MNR X MND X X X X X
RESULTS OF THE LCA - ENVIRONMENTAL IMPACT according to EN 15804+A2: 1 piece KTC 2
Parameter Unit A1-A3 A4 A5 B6 C1 C2 C3 C4 D
GWP-total kg CO 2 eq 2.15E+04 2.14E+01 8.87E+01 1.74E+04 0 1.06E+01 2.68E+02 1.39E+01 -5.32E+03
GWP-fossil kg CO 2 eq 2.17E+04 2.04E+01 1.96E+01 1.74E+04 0 1.01E+01 1.2E+02 1.38E+01 -5.31E+03
GWP-biogenic kg CO 2 eq -2.09E+02 9.45E-01 6.91E+01 -6.22E+00 0 4.66E-01 1.47E+02 4.7E-02 -1.63E+01
GWP-luluc kg CO 2 eq 5.56E+00 4.87E-04 2E-03 2.31E+01 0 2.4E-04 8E-03 4E-02 -8.88E-01
ODP kg CFC11 eq 1.42E-08 2.16E-15 2.18E-14 5.3E-11 0 1.07E-15 7.77E-14 5.13E-14 -4.04E-08
AP mol H+ eq 1.23E+02 2E-02 2.3E-02 1.45E+02 0 1E-02 4.2E-02 9.9E-02 -1.99E+01
EP-freshwater kg P eq 9.14E-03 4.38E-06 3.93E-06 1E-02 0 2.16E-06 1.22E-05 2.37E-05 -3E-03
EP-marine kg N eq 2E+01 7E-03 8E-03 1.99E+01 0 3E-03 1.2E-02 2.6E-02 -2.64E+00
EP-terrestrial mol N eq 2.19E+02 7.2E-02 1.04E-01 2.18E+02 0 3.6E-02 1.97E-01 2.8E-01 -2.86E+01
kg NMVOC
POCP 5.92E+01 1.8E-02 2.1E-02 5.96E+01 0 9E-03 3.2E-02 7.7E-02 -8.39E+00
eq
ADPE kg Sb eq 1.05E-01 6.13E-07 3.25E-07 1E-03 0 3.03E-07 1.11E-06 1.24E-06 -2E-02
ADPF MJ 2.16E+05 2.9E+02 3.06E+01 1.86E+05 0 1.43E+02 8.68E+01 1.81E+02 -7.49E+04
m3 world eq
WDP 3.14E+03 4E-02 1.06E+01 3.52E+03 0 2E-02 2.75E+01 1.45E+00 -2.63E+02
deprived
GWP = Global warming potential; ODP = Depletion potential of the stratospheric ozone layer; AP = Acidification potential of land and water; EP =
Eutrophication potential; POCP = Formation potential of tropospheric ozone photochemical oxidants; ADPE = Abiotic depletion potential for non-fossil
resources; ADPF = Abiotic depletion potential for fossil resources; WDP = Water (user) deprivation potential)
RESULTS OF THE LCA - INDICATORS TO DESCRIBE RESOURCE USE according to EN 15804+A2: 1 piece KTC 2
Parameter Unit A1-A3 A4 A5 B6 C1 C2 C3 C4 D
PERE MJ 1.62E+04 9.14E-01 6.06E+02 3.28E+04 0 4.51E-01 1.5E+03 2.38E+01 -3.45E+04
PERM MJ 2.08E+03 0 -6E+02 0 0 0 -1.48E+03 0 0
PERT MJ 1.82E+04 9.14E-01 6.21E+00 3.28E+04 0 4.51E-01 2.02E+01 2.38E+01 -3.45E+04
PENRE MJ 2.14E+05 2.9E+02 3.32E+02 1.86E+05 0 1.43E+02 1.72E+03 1.81E+02 -7.5E+04
PENRM MJ 1.94E+03 0 -3.01E+02 0 0 0 -1.64E+03 0 0
PENRT MJ 2.16E+05 2.9E+02 3.06E+01 1.86E+05 0 1.43E+02 8.68E+01 1.81E+02 -7.5E+04
SM kg 4.18E+02 0 0 0 0 0 0 0 0
RSF MJ 0 0 0 0 0 0 0 0 0
NRSF MJ 0 0 0 0 0 0 0 0 0
FW m3 7.95E+01 2E-03 2.5E-01 9.35E+01 0 8.1E-04 6.51E-01 4.6E-02 -6.11E+01
PERE = Use of renewable primary energy excluding renewable primary energy resources used as raw materials; PERM = Use of renewable primary
energy resources used as raw materials; PERT = Total use of renewable primary energy resources; PENRE = Use of non-renewable primary energy
excluding non-renewable primary energy resources used as raw materials; PENRM = Use of non-renewable primary energy resources used as raw
materials; PENRT = Total use of non-renewable primary energy resources; SM = Use of secondary material; RSF = Use of renewable secondary fuels;
NRSF = Use of non-renewable secondary fuels; FW = Use of net fresh water
RESULTS OF THE LCA – WASTE CATEGORIES AND OUTPUT FLOWS according to EN 15804+A2:
1 piece KTC 2
Parameter Unit A1-A3 A4 A5 B6 C1 C2 C3 C4 D
HWD kg 6.63E-04 2.82E-08 6.44E-08 1.13E-04 0 1.39E-08 2.31E-07 2.77E-06 -3.5E-04
NHWD kg 3.38E+03 3E-02 4.07E+00 7.14E+01 0 1.5E-02 1.33E+01 9.12E+02 -1.32E+03
RWD kg 1.49E+00 3.12E-04 1E-03 2.46E+00 0 1.54E-04 4E-03 2E-03 -8.21E+00
CRU kg 0 0 0 0 0 0 0 0 0
MFR kg 0 0 0 0 0 0 1.37E+03 0 0
MER kg 0 0 0 0 0 0 0 0 0
EEE MJ 0 0 1.4E+02 0 0 0 4.34E+02 0 0
EET MJ 0 0 2.7E+02 0 0 0 8.88E+02 0 0
5 Environmental Product Declaration - dormakaba - Automatic revolving door KTC 2
HWD = Hazardous waste disposed; NHWD = Non-hazardous waste disposed; RWD = Radioactive waste disposed; CRU = Components for re-use;
MFR = Materials for recycling; MER = Materials for energy recovery; EEE = Exported electrical energy; EET = Exported thermal energy
RESULTS OF THE LCA – additional impact categories according to EN 15804+A2-optional:
1 piece KTC 2
Parameter Unit A1-A3 A4 A5 B6 C1 C2 C3 C4 D
Disease
PM 3.02E-03 1.08E-07 1.5E-07 2E-03 0 5.31E-08 3.76E-07 1.23E-06 -3.2E-04
incidence
IR kBq U235 eq 1.98E+02 4.5E-02 2.1E-01 2E+02 0 2.2E-02 4.73E-01 2.12E-01 -1.66E+03
ETP-fw CTUe 1.02E+05 2.06E+02 1.37E+01 3.72E+04 0 1.01E+02 3.45E+01 1.04E+02 -2.75E+04
HTP-c CTUh 2.52E-05 3.87E-09 8.3E-10 3.37E-06 0 1.91E-09 2.71E-09 1.54E-08 -1.34E-06
HTP-nc CTUh 2.46E-04 1.65E-07 5.15E-08 1.53E-04 0 8.16E-08 2.12E-07 1.69E-06 -3.9E-05
SQP SQP 2.6E+04 7.45E-01 8.41E+00 2.87E+04 0 3.68E-01 2.53E+01 3.78E+01 -2.25E+03
PM = Potential incidence of disease due to PM emissions; IR = Potential Human exposure efficiency relative to U235; ETP-fw = Potential comparative
Toxic Unit for ecosystems; HTP-c = Potential comparative Toxic Unit for humans (cancerogenic); HTP-nc = Potential comparative Toxic Unit for humans
(not cancerogenic); SQP = Potential soil quality index
Disclaimer 1 – for the indicator “Potential Human exposure efficiency relative to U235”. This impact category deals mainly with the
eventual impact of low-dose ionizing radiation on human health of the nuclear fuel cycle. It does not consider effects due to possible
nuclear accidents, occupational exposure or radioactive waste disposal in underground facilities. Potential ionizing radiation from the
soil, radon and from some construction materials is also not measured by this indicator.
Disclaimer 2 – for the indicators “abiotic depletion potential for non-fossil resources”, “abiotic depletion potential for fossil resources”,
“water (user) deprivation potential, deprivation-weighted water consumption”, “potential comparative toxic unit for ecosystems”,
“potential comparative toxic unit for humans – cancerogenic”, “Potential comparative toxic unit for humans - not cancerogenic”,
“potential soil quality index”. The results of this environmental impact indicator shall be used with care as the uncertainties on these
results are high as there is limited experience with the indicator.
This EPD was created using a software tool.
References
DIN 18650 ROHS3 Directive
DIN 18650-1:2010, Powered pedestrian doors Part 1: Directive 2011/65/EU of the European Parliament and of the
Product requirements and test methods Council of 8 June 2011 on the restriction of the use of certain
hazardous substances in electrical and electronic equipment
DIN 18650
DIN 18650-2:2010, Powered pedestrian doors Part 2: IBU 2021
Safety at powered pedestrian doors General Instructions for the EPD programme of Institut Bauen
und Umwelt e.V. Version 2.0, Berlin: Institut Bauen
EN 16005 und Umwelt e.V., 2021. www.ibu-epd.com
EN 16005: 2013-01, Power operated pedestrian
doorsets - Safety in use Requirements and test methods GaBi
Sphera Solutions GmbH
EN 60335 Gabi Software System and Database for Life Cycle
EN 60335-1, 2103:2020-08, Household and Engineering 1992-2020
similar electrical appliances - Safety - Part 1: General Version 10.0.0.71
requirements University of Stuttgart
Leinfelden Echterdingen
EN 61000
EN 61000-1-2: 2017-07, Electromagnetic GaBi ts documentation
compatibility (EMC) Part 1-2: General - Methodology GaBi life cycle inventory data documentation
for the achievement of functional safety of electrical (https://www.gabisoftware.
and electronic systems including equipment with com/support/gabi/gabidatabase
regard to electromagnetic phenomena 2020lcidocumentation/)
ISO 13849 LCA-tool dormakaba
ISO 13849-1:2021-08, Safety of machinery - LCA tool, version ENS (doors)
Safety-related parts of control systems - Part 1: Tool No.: IBU-DOR-202107-LT1-EN
General principles for design Developed by Sphera Solutions GmbH
Machinery Directive PCR Part A
Directive 2006/42/EC of the European Parliament and PCR – Part A: Calculation Rules for the Life Cycle Assessment
of the Council on machinery, and amending and Requirements on the Project Report according to
Directive 95/16/EC EN 15804+A2:2019, Version 1.0, Institut
Bauen und Umwelt e.V., www.ibu-epd.com.
REACH
Regulation (EC) No 1907/2006 of the European Parliament and PCR Part B
of the Council on the Registration, Evaluation, Authorisation PCR – Part B for Automatic doors, automatic gates, and
and Restriction of Chemicals (REACH) revolving door systems,
08.2021, Institut Bauen und Umwelt e.V., www.ibu-epd.com.
6 Environmental Product Declaration - dormakaba - Automatic revolving door KTC 2
Publisher
Institut Bauen und Umwelt e.V. +49 (0)30 3087748- 0
Hegelplatz 1 info@ibu-epd.com
10117 Berlin www.ibu-epd.com
Germany
Programme holder
Institut Bauen und Umwelt e.V. +49 (0)30 3087748- 0
Hegelplatz 1 info@ibu-epd.com
10117 Berlin www.ibu-epd.com
Germany
Author of the Life Cycle Assessment
dormakaba International Holding GmbH +49 2333 793-0
DORMA Platz 1 info.de@dormakaba.com
58256 Ennepetal www.dormakaba.com
Germany
Owner of the Declaration
dormakaba International Holding GmbH +49 2333 793-0
DORMA Platz 1 info.de@dormakaba.com
58256 Ennepetal www.dormakaba.com
Germany
7 Environmental Product Declaration - dormakaba - Automatic revolving door KTC 2
