ENVIRONMENTAL PRODUCT DECLARATION
as per ISO 14025 and EN 15804+A2
Owner of the Declaration Knauf Ceiling Solutions GmbH & Co. KG
Publisher Institut Bauen und Umwelt e.V. (IBU)
Programme holder Institut Bauen und Umwelt e.V. (IBU)
Declaration number EPD-KNA-20230066-IAC1-EN
Issue date 17.04.2023
Valid to 16.04.2028
Bioguard Acoustic, Ultima
Knauf Ceiling Solutions GmbH & Co. KG
www.ibu-epd.com | https://epd-online.com
1. General Information
Knauf Ceiling Solutions GmbH & Co. KG Bioguard Acoustic, Ultima
Programme holder Owner of the declaration
IBU – Institut Bauen und Umwelt e.V. Knauf Ceiling Solutions GmbH & Co. KG
Hegelplatz 1 Elsenthal 15
10117 Berlin 94481 Grafenau
Germany Germany
Declaration number Declared product / declared unit
EPD-KNA-20230066-IAC1-EN 1 m² Bioguard Acoustic/Ultima acoustic board mineral ceiling tiles with a
surface weight of 5.53 kg/m².
This declaration is based on the product category rules: Scope:
Mineral panels, 01.08.2021 This document refers to 1 m² Bioguard Acoustic/Ultima mineral ceiling tiles
(PCR checked and approved by the SVR) with a surface weight of 5.53 kg/m², manufactured at the production facility
in Wujiang, China.
The owner of the declaration shall be liable for the underlying information
Issue date and evidence; the IBU shall not be liable with respect to manufacturer
information, life cycle assessment data and evidences.
17.04.2023
The EPD was created according to the specifications of EN 15804+A2. In
the following, the standard will be simplified as EN 15804.
Valid to
16.04.2028 Verification
The standard EN 15804 serves as the core PCR
Independent verification of the declaration and data according to ISO
14025:2011
internally X externally
Dipl.-Ing. Hans Peters
(Chairman of Institut Bauen und Umwelt e.V.)
Florian Pronold Prof. Dr. Birgit Grahl,
(Managing Director Institut Bauen und Umwelt e.V.) (Independent verifier)
1 Environmental Product Declaration - Knauf Ceiling Solutions GmbH & Co. KG - Bioguard Acoustic, Ultima
2. Product
categories 1A or 1B which are not on the candidate list,
2.1 Product description/Product definition exceeding 0.1 percentage by mass: No.
The ceiling tiles are manufactured using a wet-felt process and
consist of biosoluble mineral wool, perlite, clay and starch. In Biocide products were added to this construction product or it
addition, the visible side of the mineral tile is laminated with has been treated with biocide products (this then concerns a
glass fleece (glued), and painted with dispersion paint. The treated product as defined by the (EU) Ordinance on Biocide
back side is primed only with a dispersion paint (no glass Products No. 528/2012): No.
fleece).
In-can preservatives are used in the production process;
The mineral tiles are available in different formats and edge however, they are not part of the products and are therefore not
finishes. within the scope of the Ordinance on Biocide Products.
This EPD applies to the following products: 2.6 Manufacture
Bioguard Acoustic, Ultima The mineral tiles are produced in the traditional wet process
For the use and application of the product, the respective (wet-felt). The raw materials are mixed with water to form a
national provisions at the place of use apply, in Germany for homogeneous suspension, which is pumped onto a belt
example the building codes of the federal states and the conveyor (Fourdrinier). The water is removed mechanically
corresponding national specifications. (gravity and vacuum) and by evaporation in the drying oven. As
far as possible, the process water is reused. It is treated
2.2 Application accordingly and fed back into the process water circuit.
Mineral tiles (wet-felt) are typically used as lay-in for suspended Production waste and dust are reused in the process in the
ceiling constructions. They are primarily used as optical sense of an internal cycle. The manufacturing plant is certified
cladding, but also for sound absorption and sound insulation, according to ISO 9001, ISO 14001 and ISO 45001.
for fire resistance and against fire spreading, for cleanrooms
and high hygiene requirements. 2.7 Environment and health during manufacturing
• The manufacturing plant is certified according to ISO
2.3 Technical Data
9001, ISO 14001 and ISO 45001.
• The production has a closed water cycle.
Construction data • Production generates almost no waste, resulting blanks,
Name Value Unit dust and rejects are reused.
• Not subject to declaration according to REACH.
Noise reduction coefficient acc. ISO 354 and
0.70
ASTM C 423-01
2.8 Product processing/Installation
Airborne Sound Attenuation acc. ISO 10848 and
43 dB There are no recognised systemic hazards associated with the
ASTM E413-10
installation of ceiling tiles. It is recommended that materials are
Formaldehyde emissions (after 28 Days) < 3 µg/m³ handled in a manner that minimises dust generation. Workers
Performance data of the product with respect to its should wear appropriate personal protective equipment.
characteristics in accordance with the relevant technical Equipment such as gloves, goggles and dust masks are
provision (no CE-marking). recommended to minimise exposure to dust and prevent skin
irritation.
2.4 Delivery status
2.9 Packaging
The EPD refers to panels with a thickness of 19 mm which can
have variable length and width dimensions. The panels are packaged in cardboard boxes and sealed with
transparent polyethylene film. These packages lie on
2.5 Base materials/Ancillary materials chemically untreated wooden pallets. The pallets are wrapped
with polyethylene stretch film. Foil, paper and wood can be
Mineral tile composition:
recycled in the usual ways.
Name Value Unit
Mineral wool 26 % 2.10 Condition of use
Perlite 23 % When handled properly, the mechanical and structural-physical
properties of the mineral tile remain intact throughout its entire
Clay 17 %
service life. Direct contact with water should be avoided due to
Paper 4 %
the water-soluble binding agent starch.
Starch 5 %
2.11 Environment and health during use
Brokes/dust (internally looped production waste) 25 %
When properly installed, no dust/particles are released during
In addition, the visible side of the mineral tile is laminated with
the use phase. For the substance groups formaldehyde, volatile
glass fleece (glued) and painted with dispersion paint. The back
organic compounds (VOCs) and total volatile organic
side is primed only with a dispersion paint (no glass fleece).
compounds (TVOCs), the limits according to DIN 18177 are
The recycled content is not less than 30 %.
complied with.
This product/article/at least one partial article contains 2.12 Reference service life
substances listed in the ECHA-candidate list (date: 25.06.2020) The service life of the mineral tiles (wet-felted) is up to 50
exceeding 0.1 percentage by mass: No. years, depending on the area of use, exposure and state of
maintenance. Within the framework of the conditions of use, no
This product/article/at least one partial article contains other ageing effects are to be expected apart from visual
carcinogenic, mutagenic, reprotoxic (CMR) substances in discolouration caused by air circulation.
2 Environmental Product Declaration - Knauf Ceiling Solutions GmbH & Co. KG - Bioguard Acoustic, Ultima
demand (COD) and biological oxygen demand (BOD).
2.13 Extraordinary effects
Fire Mechanical destruction
The declared products are classified in accordance with the The mineral slabs (wet-felt) can be broken by hand and also
New Zealand Building Code and NCC Australia. damaged superficially, which can result in minor dust formation.
2.14 Re-use phase
Name Value
If the panels are removed properly, they can be reinstalled. In
NZBC Verification Method C/VM2 Group Number
case of minor damage, the slabs can be reused as cut-to-size
Appendix A Classification: 1-S
tiles. Mineral tiles can be returned to the manufacturing process
NCC 2019: Volume One Specification
Group Number if they are of the correct type and have sufficient material
C1.10 Clause 4 determined in accordance
Classification: 1 quality; they can be recycled up to 100 %.
with AS 5637.1:2015
NCC 2022: Volume One Specification 2.15 Disposal
Group Number
S7C4 determined in accordance with AS The waste code number of production residues for mineral tiles
Classification: 1
5637.1:2015 according to the AVV, German List of Wastes Ordinance is 10
11 03, the waste code number for construction site waste
(offcuts) is 17 06 04. If the tiles are not recycled as described in
Water
2.14., they are disposed of in a landfill.
In the case of prolonged contact with water, the starch binder
dissolves, which can lead to a loss of structure, and if the 2.16 Further information
soluble components are discharged into the sewage treatment
Further information at www.knaufceilingsolutions.com
plant, they are biodegradable, increasing the chemical oxygen
3. LCA: Calculation rules
declaring a 50 km radius to the landfill. In reality, this scenario
3.1 Declared Unit may vary depending on the actual location of deconstruction
This EPD refers to a declared unit of 1 m² Bioguard and referring waste treatment.
Acoustic/Ultima acoustic board mineral ceiling tiles with a
surface weight of 5.53 kg/m². Module C3 | Waste processing
The declared scenario assumes landfilling of the product.
Declared Unit Referring environmental impacts are accounted for in module
C4.
Name Value Unit
Declared unit 1 m2 Module C4 | Disposal
Grammage (with coating) 5.53 kg/m² Module C4 refers to the emissions from the disposal of the
Layer thickness 19 mm acoustic board mineral ceiling tiles. The chosen scenario,
therefore, includes the environmental burdens of landfilling the
Boardmill density (raw board, without coating) 260 kg/m³
product.
The ceiling tiles are produced at the Knauf Ceiling Solutions
production site in Wujiang, China. Module D | Benefits and loads beyond the system
Various types of mineral ceiling tiles are produced at the site. boundary
The declared product is based on the analyses of the two The declared scenario assumes landfilling of the product.
specific products Ultima and Bioguard Acoustic with the same Referring environmental impacts are accounted for in module
board formula. The acoustic board products are coated with a C4.
glass fleece facing.
3.3 Estimates and assumptions
3.2 System boundary
Assumptions and approximations are applied in case of a lack
The life cycle assessment of Bioguard Acoustic/Ultima acoustic of representative data. All assumptions and approximations are
board mineral ceiling tiles includes a cradle-to-gate analysis of documented precisely and represent a best-guess
the products' environmental impacts with modules (A1–A3, C, representation of reality. In case of uncertainty, a conservative
D). Subsequent life cycle phases are part of the analysis: approach is chosen.
Module A1–A3 | Production stage This study builds on Chinese background data as far as
The production stage includes the upstream burdens of raw supported by the available databases. Nevertheless, some
material supply, their transports and the manufacturing plant of upstream supply chains of used raw materials were
Knauf Ceiling Solutions located in Wujiang (China). Acoustic approximated via European data, due to a lack of
board mineral ceiling tiles are produced in the wet-felt process. geographically adapted datasets.
Main raw material inputs, therefore, refer to mineral wool,
perlite, clay and starch. The production site is supplied with 3.4 Cut-off criteria
electricity from the Chinese power grid and thermal energy from The LCA model covers all available input and output flows,
natural gas. which can be represented based on robust data. Data gaps are
filled with conservative assumptions from average data (when
Module C1 | Deconstruction and demolition available) or with generic data and are documented
Disassembly of the product is done either manually or using accordingly. Only data with a contribution lower than 1 % were
smaller tools. Referring energy demand is considered to be cut off. Thus, no data were neglected, of which a substantial
negligible. impact is to be expected. All relevant data were collected
comprehensively. Cut-off material and energy flows were
Modul C2 | Transport to disposal chosen carefully based on their expected quantitative
The transport to the disposal of the material is estimated contribution as well as potential environmental impacts. Thus, it
3 Environmental Product Declaration - Knauf Ceiling Solutions GmbH & Co. KG - Bioguard Acoustic, Ultima
can be assumed that the sum of all neglected input flows does basis.
not account for more than 5 % of the total material, water and
energy flows. 3.8 Geographic Representativeness
Land or region, in which the declared product system is
3.5 Background data manufactured, used or handled at the end of the product´s
This study uses generic background data for the evaluation of lifespan: China
upstream environmental impacts from GaBi databases (GaBi
10; 2022.2).
3.9 Allocation
3.6 Data quality All information for the allocation of given material and energy
Data collection is based on product-specific questionnaires. It flows is based on site-related evaluations. The calculation of
follows an iterative process of clarifying questions via e-mail, specific input quantities for the raw board production is based
telephone calls or in personal/web-meetings. Intensive on the respective recipe. In addition, product-specific
discussions between Knauf Ceiling Solutions and Daxner & application rates (e.g. backcoat, primer, glass fleece etc.) were
Merl result in an accurate mapping of product-related material available. Total annual energy consumption and waste flows
and energy flows. This leads to a high quality of foreground are allocated based on the production share of the product.
data collected. Data collection relies on a consistent process
according to ISO 14044. For in the production used waste paper, the system boundary is
set after sorting. It is assumed that the end of waste status has
The technological, geographical and time-related been reached. The system boundary for secondary raw
representativeness of the database was kept in mind when materials defined in EN 15804 applies.
selecting background data. Whenever specific data were
3.10 Comparability
missing, either generic datasets or representative average data
were used instead. The implemented GaBi background Basically, a comparison or an evaluation of EPD data is only
datasets refer to the latest versions available (not more than possible if all the data sets to be compared were created
ten years old) and are carefully chosen. according to EN 15804 and the building context, respectively
the product-specific characteristics of performance, are taken
3.7 Period under review into account. The GaBi background database was used to
Foreground data were collected in the 2021 production year, calculate the LCA (GaBi 10; 2022.2).
and the data are based on the volumes produced on an annual
4. LCA: Scenarios and additional technical information
Characteristic product properties of biogenic carbon
The biogenic carbon content quantifies the amount of biogenic
carbon in the declared product.
Installation in building (A5)
Information on the description of the biogenic carbon The End-of-Life of the product packaging materials is not
content at the factory gate declared in module A5.
Name ValueUnit Name Value Unit
Biogenic carbon content in product 0.24 kg Packaging (cardboard) 0.009 kg/m²
C
Packaging (PE-film) 0.035 kg/m²
Biogenic carbon content in accompanying kg
0.015
packaging C
End-of-Life (C1-C4)
The carbon stored in the packaging was taken into account as
"CO -neutral". Thus the storage effect of the carbon bound in Name Value Unit
2
the packaging is not included in the calculation but is Collected separately 5.53 kg
considered as emitted immediately. Landfilling 5.53 kg
4 Environmental Product Declaration - Knauf Ceiling Solutions GmbH & Co. KG - Bioguard Acoustic, Ultima
5. LCA: Results
The following table contains the LCA results for a declared unit of 1 m² Bioguard Acoustic/Ultima acoustic board mineral ceiling tiles
with a surface weight of 5.53 kg/m².
DESCRIPTION OF THE SYSTEM BOUNDARY (X = INCLUDED IN LCA; ND = MODULE OR INDICATOR NOT DECLARED; MNR =
MODULE NOT RELEVANT)
Benefits and
Construction loads beyond
Product stage Use stage End of life stage
process stage the system
boundaries
la ire ta m w a Ry lp p u s tro p s n a rT g n iru tc a fu n a M e h t m o rf tro p s n a rTe tis e h t o t e ta g y lb m e s s A e s U e c n a n e tn ia M ria p e R tn e m e c a lp e R tn e m h s ib ru fe R y g re n e la n o ita re p Oe s u re ta w la n o ita re p Oe s u n o itc u rts n o c -e Dn o itilo m e d tro p s n a rT g n is s e c o rp e ts a W la s o p s iD -e s u e R-y re v o c e R-g n ilc y c e Rla itn e to p
A1 A2 A3 A4 A5 B1 B2 B3 B4 B5 B6 B7 C1 C2 C3 C4 D
X X X MND MND MND MND MNR MNR MNR MND MND X X X X X
RESULTS OF THE LCA - ENVIRONMENTAL IMPACT according to EN 15804+A2: 1 m² Bioguard Acoustic/Ultima acoustic
boards (5.53 kg/m²)
Parameter Unit A1-A3 C1 C2 C3 C4 D
Global Warming Potential total (GWP-total) kg CO 2 eq 6.39E+00 0 1.73E-02 0 9.71E-01 0
Global Warming Potential fossil fuels (GWP-fossil) kg CO 2 eq 7.23E+00 0 1.66E-02 0 8.25E-02 0
Global Warming Potential biogenic (GWP-biogenic) kg CO 2 eq -8.48E-01 0 7.35E-04 0 8.88E-01 0
Global Warming Potential luluc (GWP-luluc) kg CO 2 eq 1.65E-03 0 4.32E-07 0 1.52E-04 0
Depletion potential of the stratospheric ozone layer (ODP) kg CFC11 eq 2.11E-10 0 1.63E-15 0 1.94E-13 0
Acidification potential of land and water (AP) mol H+ eq 3.29E-02 0 5.57E-05 0 5.85E-04 0
Eutrophication potential aquatic freshwater (EP-freshwater) kg P eq 1.26E-04 0 2.09E-09 0 1.4E-07 0
Eutrophication potential aquatic marine (EP-marine) kg N eq 7.89E-03 0 2.52E-05 0 1.5E-04 0
Eutrophication potential terrestrial (EP-terrestrial) mol N eq 1.04E-01 0 2.77E-04 0 1.64E-03 0
Formation potential of tropospheric ozone photochemical oxidants kg NMVOC
1.65E-02 0 5.03E-05 0 4.55E-04 0
(POCP) eq
Abiotic depletion potential for non fossil resources (ADPE) kg Sb eq 9.88E-07 0 6.72E-10 0 8.46E-09 0
Abiotic depletion potential for fossil resources (ADPF) MJ 9.74E+01 0 2.29E-01 0 1.08E+00 0
m3 world eq
Water use (WDP) 9.36E-01 0 1.41E-04 0 9.05E-03 0
deprived
RESULTS OF THE LCA - INDICATORS TO DESCRIBE RESOURCE USE according to EN 15804+A2: 1 m² Bioguard
Acoustic/Ultima acoustic boards (5.53 kg/m²)
Parameter Unit A1-A3 C1 C2 C3 C4 D
Renewable primary energy as energy carrier (PERE) MJ 1.13E+00 0 1.24E-03 0 1.62E-01 0
Renewable primary energy resources as material utilization
MJ 1.01E+01 0 0 0 0 0
(PERM)
Total use of renewable primary energy resources (PERT) MJ 1.12E+01 0 1.24E-03 0 1.62E-01 0
Non renewable primary energy as energy carrier (PENRE) MJ 9.66E+01 0 2.3E-01 0 1.08E+00 0
Non renewable primary energy as material utilization (PENRM) MJ 9.16E-01 0 0 0 0 0
Total use of non renewable primary energy resources (PENRT) MJ 9.75E+01 0 2.3E-01 0 1.08E+00 0
Use of secondary material (SM) kg 2.52E-01 0 0 0 0 0
Use of renewable secondary fuels (RSF) MJ 0 0 0 0 0 0
Use of non renewable secondary fuels (NRSF) MJ 0 0 0 0 0 0
Use of net fresh water (FW) m3 2.99E-02 0 3.56E-06 0 2.75E-04 0
RESULTS OF THE LCA – WASTE CATEGORIES AND OUTPUT FLOWS according to EN 15804+A2:
1 m² Bioguard Acoustic/Ultima acoustic boards (5.53 kg/m²)
Parameter Unit A1-A3 C1 C2 C3 C4 D
Hazardous waste disposed (HWD) kg 4.42E-06 0 5.75E-13 0 5.56E-11 0
Non hazardous waste disposed (NHWD) kg 7.82E-01 0 9.51E-06 0 5.54E+00 0
Radioactive waste disposed (RWD) kg 1.23E-03 0 1.29E-07 0 1.2E-05 0
Components for re-use (CRU) kg 0 0 0 0 0 0
Materials for recycling (MFR) kg 0 0 0 0 0 0
Materials for energy recovery (MER) kg 0 0 0 0 0 0
Exported electrical energy (EEE) MJ 0 0 0 0 0 0
Exported thermal energy (EET) MJ 0 0 0 0 0 0
RESULTS OF THE LCA – additional impact categories according to EN 15804+A2-optional:
1 m² Bioguard Acoustic/Ultima acoustic boards (5.53 kg/m²)
Parameter Unit A1-A3 C1 C2 C3 C4 D
Disease
Incidence of disease due to PM emissions (PM) 3.02E-07 0 3E-10 0 7.2E-09 0
incidence
5 Environmental Product Declaration - Knauf Ceiling Solutions GmbH & Co. KG - Bioguard Acoustic, Ultima
Human exposure efficiency relative to U235 (IR) kBq U235 eq 1.7E-01 0 8.56E-06 0 1.33E-03 0
Comparative toxic unit for ecosystems (ETP-fw) CTUe 2.9E+01 0 2.72E-01 0 6.06E-01 0
Comparative toxic unit for humans (carcinogenic) (HTP-c) CTUh 4.16E-09 0 4.36E-12 0 9.24E-11 0
Comparative toxic unit for humans (noncarcinogenic) (HTP-nc) CTUh 8.05E-08 0 1.51E-10 0 1.02E-08 0
Soil quality index (SQP) SQP 1.52E+01 0 6.77E-04 0 2.25E-01 0
Disclaimer 1 – for the indicator Potential human exposure efficiency relative to U235:
This impact category deals mainly with the eventual impact of low dose ionizing radiation on human health of the nuclear fuel cycle. It
does not consider effects due to possible nuclear accidents, occupational exposure nor due to radioactive waste disposal in
underground facilities. Potential ionizing radiation from the soil, from radon and from some construction materials is also not measured
by this indicator.
Disclaimer 2 – for the indicators Abiotic depletion potential for non-fossil resources, Abiotic depletion potential for fossil resources,
Water (user) deprivation potential, deprivation-weighted water consumption , Potential comparative toxic unit for ecosystems, Potential
comparative toxic unit for humans - cancerogenic, Potential comparative toxic unit for humans - not cancerogenic, Potential soil quality
index: The results of this environmental impact indicator shall be used with care as the uncertainties on these results are high or as
there is limited experience with the indicator.
6. LCA: Interpretation
The following interpretation contains a summary of the LCA Acoustic/Ultima acoustic board mineral ceiling tiles.
results referenced to a functional unit of 1 m² Bioguard
The comparison of the product's life cycle phases shows a (ADPE) as well as the formation potential of tropospheric ozone
clear dominance of the production phase (modules A1–A3) in (POCP). The main contributors to water deprivation potential
all environmental impact categories. The potential (WDP) are electricity provision as well as water losses at the
environmental impacts from transport to disposal (module C2) site resulting from the evaporation of cooling water at the drying
and the End-of-Life of the products due to landfilling (module oven.
C4) have a minor contribution.
For most impact categories the supply of mineral wool is an
The upstream supply chain of the raw board plays a dominant important influencing factor in the raw board composition.
role in all categories except for abiotic depletion potential for
fossil resources (ADPF) and water deprivation potential (WDP). As the declared Bioguard Acoustic/Ultima acoustic board
Furthermore, thermal energy provision at the site represents a mineral ceiling tiles share the same board formula as well as
major contributor to global warming potential (GWP), potential surface weight, there is no variance of the results.
depletion of fossil resources (ADPF), abiotic depletion potential
7. Requisite evidence
Not applicable for these products.
7.1 Radioactivity 7.2 Biopersistence
6 Environmental Product Declaration - Knauf Ceiling Solutions GmbH & Co. KG - Bioguard Acoustic, Ultima
The mineral wool used for the production of the panels is Testing period: 16/09/2022 - 14/10/2022
biosoluble. Test basis: ISO 16000-6
Measuring point: Fraunhofer Institute for Toxicology and
Test after 28 days
Experimental Medicine
Name Value Unit
Certificate number: 02G15015 (5 September 2016)
Test substance: Slag Wool 'Arm SW15' TVOC < 9.5 μg/m³
7.3 VOC emissions TSVOC < 12 μg/m³
Measuring point: Eurofins Product Testing A/S R (dimensionless) 0
Test reports: VOC emission test report Indoor Air Comfort
Sum of VOC without NIK/LCI < 5 μg/m³
GOLD (20 October 2022)
Carcinogenic substances < 1 μg/m³
Numbers:
392-2022-00399102_A_EN Formaldehyde < 3 µg/m³
392-2022-00399101_A_EN
8. References
Standards Absorption and Sound Absorption Coefficients by the
Reverberation Room Method.
DIN 18177
DIN 18177:2020-12, Wet-felt factory-produced mineral panels. ASTM E413-10
ASTM E413-10:2010-09, Classification for Rating Sound
EN 15804 Insulation.
DIN EN 15804:2012+A2:2019+AC:2021, Sustainability of
construction works – Environmental product declarations – Further References
Core rules for the product category of construction products.
AVV, German List of Wastes Ordinance
ISO 354 Regulation on the European Waste List. Waste Catalogue
DIN EN ISO 354:2003-12, Acoustics – Measurement of sound Ordinance (German designation: Abfallverzeichnisverordnung –
absorption in reverberant rooms. AVV) of 10 December 2001 (Federal Law Gazette I p. 3379),
last amended by Article 1 of the Ordinance of 30 June 2020
ISO 717-1 (Federal Law Gazette I p. 3005).
DIN EN ISO 717-1:2013-06, Acoustics – Assessment of sound
insulation in buildings and of building elements – Part 1: Chemicals Prohibition Ordinance
Airborne sound insulation. Chemicals Prohibition Ordinance (German designation:
Chemikalien-Verbotsverordnung – ChemVerbotsV) of 20
ISO 9001 January 2017 (Federal Law Gazette I p. 94; 2018 I p. 1389),
DIN EN ISO 9001:2015-11, Quality management systems – last amended by Article 300 of the Ordinance of 19 June 2020
Requirements. (Federal Law Gazette I p. 1328).
ISO 10848 ECHA-candidate list
DIN EN ISO 10848-2:2006-08, Acoustics – Measurement of List of substances of very high concern (SVHC) for
airborne and impact sound transmission between adjacent authorisation (ECHA Candidate List), 25.06.2020, published
rooms in test stands – Part 2: Application to lightweight under Article 59(10) of REACH. Helsinki: European Chemicals
components where the connection has a minor influence. Agency.
ISO 14001 Eurofins Product Testing A/S
DIN EN ISO 14001:2015-11, Environmental management Test report:VOC emission test report Indoor Air Comfort GOLD
systems – Requirements with guidance for use. (20 October 2022). Numbers: 392-2022-00399102_A_EN, 392-
2022-00399101_A_EN.
ISO 14025
DIN EN ISO 14025:2011-10, Environmental labels and Fraunhofer Institute for Toxicology and Experimental
declarations – Type III environmental declarations – Principles Medicine
and procedures. Certificate number: 02G15015 (5 September 2016); Test
substance: Slag Wool 'Arm SW15'.
ISO 14044
DIN EN ISO 14044:2006-10, Environmental management – Life GaBi
cycle assessment – Requirements and guidelines. GaBi 10, Software-System and Database for Life Cycle
Engineering. DB 2022.2. Sphera, 1992–2022. Available at:
ISO 16000-6 https://gabi.sphera.com/support/gabi/
ISO 16000-6:2011-12, Indoor air contaminants – Part 6:
Determination of VOCs in indoor air and test chambers, NCC Australia
sampling on Tenax TA®, thermal desorption and gas Initiative of the Council of Australian Governments, developed
chromatography with MS/FID. to incorporate all on-site construction requirements into a single
code. Available at: https://ncc.abcb.gov.au/
ISO 45001
DIN ISO 45001:2018-06, Occupational health and safety NCC 2019
management systems – Requirements with guidance for use. NCC 2019: Volume One Specification C1.10 Clause 4
determined in accordance with AS 5637.1:2015.
ASTM C423-01
ASTM C423-01:2001-07, Standard Test Method for Sound NCC 2022
7 Environmental Product Declaration - Knauf Ceiling Solutions GmbH & Co. KG - Bioguard Acoustic, Ultima
NCC 2022: Volume One Specification S7C4 determined in IBU 2021
accordance with AS 5637.1:2015. Institut Bauen und Umwelt e.V.: General instructions for the
EPD programme of Institut Bauen und Umwelt e.V. (IBU).
New Zealand Building Code Version 2.0, Berlin: Institut Bauen und Umwelt e.V., 2021.
The Building Code is contained in regulations under the www.ibuepd.com
Building Act 2004. The Act governs the building sector and also
sets out the rules for the construction, alteration, demolition and PCR Part A
maintenance of new and existing buildings in New Zealand. It Product category rules for building-related products and
works alongside other legislation for health, safety, consumer services. Part A: Calculation rules for the life cycle assessment
protection and land use. Available at: and requirements on the project report according to
www.building.govt.nz/building-code-compliance/building-code- EN15804+A2:2019. Version 1.3, Berlin: Institut Bauen und
and-handbooks/ Umwelt e.V. (Hrsg.), 2022.
Ordinance on Biocide Products PCR: Mineral panels
Regulation (EU) No 528/2012 of the European Parliament and Institut Bauen und Umwelt e.V. (IBU), 2019. Product Category
of the Council of 22 May 2012 concerning the making available Rules for Building-Related Products and Services. Part B:
on the market and use of biocidal products. Requirements on the EPD for Mineral panels. 08.03.2023.
Ordinance on Hazardous Substances REACH
Ordinance on Hazardous Substances, of 26 November 2010 Regulation (EC) No 1907/2006 of the European Parliament and
(Federal Law Gazette I p. 1643, 1644), last amended by Article Council from 18 December 2006, Regulation concerning the
148 of the Law of 29 March 2017 (Federal Law Gazette I p. Registration, Evaluation, Authorisation and Restriction of
626). Chemicals (REACH).
8 Environmental Product Declaration - Knauf Ceiling Solutions GmbH & Co. KG - Bioguard Acoustic, Ultima
Publisher
Institut Bauen und Umwelt e.V. +49 (0)30 3087748- 0
Hegelplatz 1 info@ibu-epd.com
10117 Berlin www.ibu-epd.com
Germany
Programme holder
Institut Bauen und Umwelt e.V. +49 (0)30 3087748- 0
Hegelplatz 1 info@ibu-epd.com
10117 Berlin www.ibu-epd.com
Germany
Author of the Life Cycle Assessment
Daxner & Merl GmbH +43 676 849477826
Lindengasse 39/8 office@daxner-merl.com
1070 Wien www.daxner-merl.com
Austria
Owner of the Declaration
Knauf Ceiling Solutions GmbH & Co. KG 0049 8552 422 0
Elsenthal 15 info@knaufamf.com
94481 Grafenau www.knaufceilingsolutions.com
Germany
9 Environmental Product Declaration - Knauf Ceiling Solutions GmbH & Co. KG - Bioguard Acoustic, Ultima
