ENVIRONMENTAL PRODUCT DECLARATION
as per ISO 14025 and EN 15804+A2
Owner of the Declaration dormakaba International Holding GmbH
Publisher Institut Bauen und Umwelt e.V. (IBU)
Programme holder Institut Bauen und Umwelt e.V. (IBU)
Declaration number EPD-DOR-20210181-CBA2-EN
Issue date 07.10.2021
Valid to 06.10.2026
Access manager 92 30
dormakaba
www.ibu-epd.com | https://epd-online.com
General Information
dormakaba Access manager 92 30
Programme holder Owner of the declaration
IBU – Institut Bauen und Umwelt e.V. dormakaba International Holding GmbH
Hegelplatz 1 DORMA Platz 1
10117 Berlin 58256 Ennepetal
Germany Germany
Declaration number Declared product / declared unit
EPD-DOR-20210181-CBA2-EN 1 piece of the product: Access manager 92 30
This declaration is based on the product category rules: Scope:
Electronic and physical Access Control Systems, 01.08.2021 This EPD refers to a specific product manufactured by dormakaba. The
(PCR checked and approved by the SVR) production site is located in Villingen-Schwenningen (Germany).
The data represents the year 2020.
The owner of the declaration shall be liable for the underlying information
Issue date and evidence; the IBU shall not be liable with respect to manufacturer
information, life cycle assessment data and evidences.
07.10.2021
The EPD was created according to the specifications of EN 15804+A2. In
the following, the standard will be simplified as EN 15804.
Valid to
06.10.2026 Verification
The standard EN 15804 serves as the core PCR
Independent verification of the declaration and data according to ISO
14025:2011
internally X externally
Dipl.-Ing. Hans Peters
(Chairman of Institut Bauen und Umwelt e.V.)
Florian Pronold Dr.-Ing. Wolfram Trinius,
(Managing Director Institut Bauen und Umwelt e.V.) (Independent verifier)
1 Environmental Product Declaration - dormakaba - Access manager 92 30
Product
Host Interface
Product description/Product definition • Ethernet 10/100 Mbit/s
The dormakaba access manager 92 30 is a high-performance
access control system, optimised for single access points. Peripherals Interface
Thanks to its intelligent decision logic and ability to be freely Variant MRD
parametrised, the access manager can control simple types of
access as well as more complex entrance and exit door • 2x coaxial for registration units (LEGIC / MIFARE) • 1x RS-
configurations. Based on the latest operating system and TLS 485 • 1x RS-232
encryption between the controller and host system, the IT • 3x potential-free relays, 30 V AC/DC; max. 2 A • 4x digital
security is state-of-the-art. With integrated mobile access, the inputs
access system allows access via smartphone. The control • 1x tamper contact
electronics integrate everything that is required to enable a
connection to cloud services via IoT. Power supply via PoE Variant Wiegand • 2x Wiegand • 1x RS232 • 3x potential-free
allows easy integration and the compact and discreet design relays, 30 V AC/DC; max. 2 A • 4x digital inputs • 1x tamper
allows installation in full view. Up to two registration units can contact
be connected directly and further access readers via the RS-
485 sub-bus. Optionally, a version with two Wiegand interfaces
offers maximum flexibility and connectivity. For the placing on Power supply
the market in the European Union/European Free Trade • PoE, as per IEEE 802.3af
Association (EU/EFTA) (with the exception of Switzerland) the • PoE+, as per IEEE 802.3at
following legal provisions apply:
Output voltage
• Electromagnetic Compatibility Directive (EMC) • Reader: 5/12 V DC • Elec. door opener: 12/24 V DC
• Low Voltage Directive (LVD)
• Restriction of Hazardous Substances (RoHS) Class of protection as per EN 60529:IP40.
• Radio Equipment Directive (RED)
• EN 50581:2012 The product is not harmonised in accordance with the
Construction Product Regulations (CPR) but in accordance with
The CE-marking takes into account the proof of conformity with other provisions for harmonisation of the EU. Compliance with
the respective harmonized standards based on the legal the European Union Directive and technical specifications:
provisions above. For the application and use the respective • EN 55032:2015
national provisions apply. • EN 55024:2010 + A1:2015
• EN 50364:2010
Application
• EN 62368-1:2014 + A11:2017
Flexible access control • EN 60529:2014
An access manager is installed in a protected environment and • EN 301489-1 V2.2.1 Draft
uses local or online decision logic to check whether an access • EN 301489-3 V2.1.1
request via connected card readers is granted or rejected. • EN 300330 V2.1.1
The product is subject to CE marking according to the relevant
Door management harmonization legislation.
• Personnel interlock control In addition, the product also conforms to the following
• Door activation standards:
• Monitoring of door opening
• UL 294:2013
• Monitoring of door opening time
• UL62368-1:2014-12
• Access monitoring
• CAN/CSA-22.2 No. 62368-1:2014-12
• FCC ID NVI-DKAM9230K7
Alarm Management
The access manager reports irregularities in access control or
Base materials/Ancillary materials
door management to the host computer. Tampering and
The major material compositions of the product are listed
burglary attempts are reliably identified.
below:
Technical Data Name Value Unit
The access manager 92 30 has the following technical Plastics 48,5 %
properties: Paper 27 %
Name Value Unit
Electronics 23,5 %
Operating Temperature 0 - 50 °C
Steel 1 %
Operating Humidity 5 - 85 %
The product includes partial articles which contain substances
Width Dimension 208 mm
listed in the Candidate List of REACH Regulation
Height Dimension 208 mm 1907/2006/EC (date: 08.07.2021) exceeding 0.1 percentage by
Depth Dimension 48 mm mass in the alloy: yes
Weight (without packaging) 0,675 kg • Lead titanium trioxide (O3PbTi): 12060-00-03
Weight (with packaging) 0,923 kg The Candidate List can be found on the ECHA website
Power consumption "idle mode" 5 W address: https:echa.europa.eu/de/home.
Power consumption "on mode" 12 W
Reference service life
2 Environmental Product Declaration - dormakaba - Access manager 92 30
The reference service life of the dormakaba access manager support and service life and is not an estimated lifetime.
92 30 is estimated to be 15 years. This number is based on the
LCA: Calculation rules
Use stage - Module B6
Declared Unit The use stage related to the operation of the building includes:
The declared unit is 1 piece of the product: Access manager 92 — B6, operational energy use
30.
Declared unit End-of-life stage– Modules C1-C4 and D
The end-of-life stage includes:
Name Value Unit
— C1, de-construction, demolition:
Declared unit 1 pce.
— C2, transport to waste processing;
Product weight including packaging 0,923 kg — C3, waste processing for reuse, recovery and/or recycling;
— C4, disposal;
System boundary
The type of EPD is: cradle to gate with options, modules C1– including provision and all transport, provision of all materials,
C4, and module D (A1–A3 + C + D and additional modules: A4 products and related energy and water use.
+ A5 + B6)
Module D (Benefits and loads beyond the system boundary)
Production - Module A1-A3 includes:
The product stage includes: — D, recycling potentials, expressed as net impacts and
— A1, raw material extraction, processing and mechanical benefits.
treatments, processing of secondary material input (e.g.
Geographic Representativeness
recycling processes), — A2, transport to the manufacturer,
Land or region, in which the declared product system is
— A3, manufacturing and assembly including provision of all
manufactured, used or handled at the end of the product´s
materials, products and energy, as well as waste processing up
lifespan: Germany
to the end-of waste state.
Construction stage - Modules A4-A5
Comparability
The construction process stage includes:
Basically, a comparison or an evaluation of EPD data is only
— A4, transport to the building site; — A5, installation into the
possible if all the data sets to be compared were created
building; including provision of all materials, products and
according to EN 15804 and the building context, respectively
energy, as well as waste processing up to the end-of-waste
the product-specific characteristics of performance, are taken
state or disposal of final residues during the construction
into account. Background database: GaBi, SP40.
process stage.
LCA: Scenarios and additional technical information
Reference service life
Characteristic product properties of biogenic carbon
Name Value Unit
Information on describing the biogenic Carbon Content at
Life Span according to the manufacturer 15 a
factory gate
Name ValueUnit Operational energy use (B6) and Operational water use
kg (B7)
Biogenic carbon content in product 0.01
C The use stage is declared for 15 years.
Biogenic carbon content in accompanying kg Name Value Unit
0.1
packaging C
Energy consumption for 1 year 54.02 kWh
Note: 1 kg of biogenic carbon is equivalent to 44/12 kg of CO 2. on mode per day 4 h
idle mode 20 h
on mode power 12 W
The following technical scenario information is required for the
idle mode 5 W
declared modules.
Days per year in use 365 days
Transport to the building site (A4)
Name Value Unit End of life (C1-C4)
Litres of fuel per 1 kg (truck) 0.00276 l/100km C1: The product dismantling from the building is done manually
without environmental burden.
Transport distance (truck) 750 km
Capacity utilisation (including empty runs) 51 % Name Value Unit
Transort distance (ship) 1000 km Recycling (Steel) 0.01 kg
Energy recovery (Plastic) 0.43 kg
Installation into the building (A5)
Energy recovery (Paper) 0,02 kg
Name Value Unit Recycling and landfilling (Electronics) 0,21 kg
Waste Packaging (paper) 0.227 kg Transportation to Waste 50 km
Waste Packaging (plastic) 0,022 kg
Region for end of life: Global
3 Environmental Product Declaration - dormakaba - Access manager 92 30
Reuse, recovery and/or recycling potentials (D), relevant Collection rate is 100%.
scenario information
4 Environmental Product Declaration - dormakaba - Access manager 92 30
LCA: Results
DESCRIPTION OF THE SYSTEM BOUNDARY (X = INCLUDED IN LCA; MND = MODULE OR INDICATOR NOT DECLARED; MNR
= MODULE NOT RELEVANT)
Benefits and
Construction loads beyond
Product stage Use stage End of life stage
process stage the system
boundaries
la ire ta m w a Ry lp p u s tro p s n a rT g n iru tc a fu n a M e h t m o rf tro p s n a rTe tis e h t o t e ta g y lb m e s s A e s U e c n a n e tn ia M ria p e R tn e m e c a lp e R tn e m h s ib ru fe R y g re n e la n o ita re p Oe s u re ta w la n o ita re p Oe s u n o itc u rts n o c -e Dn o itilo m e d tro p s n a rT g n is s e c o rp e ts a W la s o p s iD -e s u e R-y re v o c e R-g n ilc y c e Rla itn e to p
A1 A2 A3 A4 A5 B1 B2 B3 B4 B5 B6 B7 C1 C2 C3 C4 D
X X X X X MND MND MNR MNR MNR X MND MND X X X X
RESULTS OF THE LCA - ENVIRONMENTAL IMPACT according to EN 15804+A2: 1 piece Access manager 92 30
Parameter Unit A1-A3 A4 A5 B6 C2 C3 C4 D
GWP-total kg CO 2 eq 1.59E+01 6.36E-02 3.75E-01 4.13E+02 2.98E-03 1.08E+00 4.05E-04 -1.24E+00
GWP-fossil kg CO 2 eq 1.61E+01 6.09E-02 6.16E-02 4.11E+02 2.85E-03 1.08E+00 4.02E-04 -1.24E+00
GWP-biogenic kg CO 2 eq -2.4E-01 2.68E-03 3.14E-01 8.16E-01 1.32E-04 2.53E-05 1.37E-06 1.69E-04
GWP-luluc kg CO 2 eq 2.31E-02 1.44E-06 8.32E-06 5.78E-01 6.78E-08 6.13E-05 1.16E-06 -1.45E-03
ODP kg CFC11 eq 1.75E-09 6.39E-18 8.5E-17 6.2E-12 3.01E-19 5.47E-16 1.49E-18 -8.26E-15
AP mol H+ eq 8.57E-02 1.69E-04 9.97E-05 1.83E+00 2.85E-06 1.93E-04 2.88E-06 -1.14E-02
EP-freshwater kg P eq 1.14E-04 1.31E-08 1.56E-08 7.83E-04 6.1E-10 8.73E-08 6.9E-10 -1.18E-06
EP-marine kg N eq 1.52E-02 4.78E-05 3.47E-05 3E-01 9.07E-07 4.35E-05 7.42E-07 -9.75E-04
EP-terrestrial mol N eq 1.62E-01 5.26E-04 4.49E-04 3.23E+00 1.01E-05 8.8E-04 8.16E-06 -1.05E-02
kg NMVOC
POCP 4.47E-02 1.34E-04 9.22E-05 8.67E-01 2.56E-06 1.21E-04 2.25E-06 -3.19E-03
eq
ADPE kg Sb eq 1.31E-01 1.81E-09 1.29E-09 8.48E-05 8.54E-11 7.5E-09 3.61E-11 -4.92E-04
ADPF MJ 2.07E+02 8.57E-01 1.26E-01 6.19E+03 4.04E-02 5.03E-01 5.27E-03 -1.79E+01
m3 world eq
WDP 3.51E+00 1.19E-04 4.54E-02 8.74E+01 5.58E-06 1.11E-01 4.21E-05 -3.54E-01
deprived
GWP = Global warming potential; ODP = Depletion potential of the stratospheric ozone layer; AP = Acidification potential of land and water; EP =
Eutrophication potential; POCP = Formation potential of tropospheric ozone photochemical oxidants; ADPE = Abiotic depletion potential for non-fossil
resources; ADPF = Abiotic depletion potential for fossil resources; WDP = Water (user) deprivation potential)
RESULTS OF THE LCA - INDICATORS TO DESCRIBE RESOURCE USE according to EN 15804+A2: 1 piece Access manager 92
30
Parameter Unit A1-A3 A4 A5 B6 C2 C3 C4 D
PERE MJ 4.5E+01 2.71E-03 2.75E+00 2.32E+03 1.27E-04 3.95E-01 6.91E-04 -3.05E+00
PERM MJ 4.8E+01 0 -2.72E+00 0 0 -2.64E-01 0 0
PERT MJ 2.36E+02 2.71E-03 2.49E-02 2.32E+03 1.27E-04 1.31E-01 6.91E-04 -3.05E+00
PENRE MJ 2.07E+02 8.58E-01 1.03E+00 6.2E+03 4.04E-02 1.59E+01 5.28E-03 -1.79E+01
PENRM MJ 2.24E+02 0 -9.05E-01 0 0 -1.54E+01 0 0
PENRT MJ 2.08E+02 8.58E-01 1.26E-01 6.2E+03 4.04E-02 5.03E-01 5.28E-03 -1.79E+01
SM kg 7.1E-03 0 0 0 0 0 0 0
RSF MJ 0 0 0 0 0 0 0 0
NRSF MJ 9.51E-02 0 0 0 0 0 0 0
FW m3 9.51E-02 4.86E-06 1.07E-03 3.16E+00 2.28E-07 2.65E-03 1.33E-06 -7.79E-03
PERE = Use of renewable primary energy excluding renewable primary energy resources used as raw materials; PERM = Use of renewable primary
energy resources used as raw materials; PERT = Total use of renewable primary energy resources; PENRE = Use of non-renewable primary energy
excluding non-renewable primary energy resources used as raw materials; PENRM = Use of non-renewable primary energy resources used as raw
materials; PENRT = Total use of non-renewable primary energy resources; SM = Use of secondary material; RSF = Use of renewable secondary fuels;
NRSF = Use of non-renewable secondary fuels; FW = Use of net fresh water
RESULTS OF THE LCA – WASTE CATEGORIES AND OUTPUT FLOWS according to EN 15804+A2:
1 piece Access manager 92 30
Parameter Unit A1-A3 A4 A5 B6 C2 C3 C4 D
HWD kg 1.39E-05 8.33E-11 2.44E-10 2.87E-06 3.92E-12 1.92E-09 8.04E-11 -3.1E-08
NHWD kg 5.21E-01 8.77E-05 1.56E-02 3.87E+00 4.13E-06 1.13E-01 2.65E-02 -1.4E-01
RWD kg 4.8E-03 9.22E-07 6.26E-06 7.18E-01 4.34E-08 1.87E-05 6E-08 -7.74E-04
CRU kg 0 0 0 0 0 0 0 0
MFR kg 0 0 0 0 0 2.28E-01 0 0
MER kg 0 0 0 0 0 0 0 0
EEE MJ 1.07E-01 0 5.86E-01 0 0 0 0 0
EET MJ 1.95E-01 0 1.11E+00 0 0 0 0 0
5 Environmental Product Declaration - dormakaba - Access manager 92 30
HWD = Hazardous waste disposed; NHWD = Non-hazardous waste disposed; RWD = Radioactive waste disposed; CRU = Components for re-use;
MFR = Materials for recycling; MER = Materials for energy recovery; EEE = Exported electrical energy; EET = Exported thermal energy
RESULTS OF THE LCA – additional impact categories according to EN 15804+A2-optional:
1 piece Access manager 92 30
Parameter Unit A1-A3 A4 A5 B6 C2 C3 C4 D
Disease
PM 8.63E-07 2.2E-09 6.21E-10 2.56E-05 1.5E-11 2.46E-09 3.57E-11 -9.35E-08
incidence
IR kBq U235 eq 4.65E-01 1.32E-04 9.09E-04 1.16E+02 6.2E-06 1.68E-03 6.18E-06 -1.24E-01
ETP-fw CTUe 1.35E+02 6.08E-01 5.75E-02 2.28E+03 2.86E-02 1.89E-01 3.01E-03 -6.86E+00
HTP-c CTUh 1.91E-08 1.14E-11 3.36E-12 8.34E-08 5.39E-13 1.63E-11 4.47E-13 -4.78E-10
HTP-nc CTUh 2.96E-07 4.91E-10 1.92E-10 3.32E-06 2.3E-11 1.65E-09 4.92E-11 -3.26E-08
SQP SQP 7.6E+01 2.21E-03 3.44E-02 1.71E+03 1.04E-04 1.51E-01 1.1E-03 -6.06E+00
PM = Potential incidence of disease due to PM emissions; IR = Potential Human exposure efficiency relative to U235; ETP-fw = Potential comparative
Toxic Unit for ecosystems; HTP-c = Potential comparative Toxic Unit for humans (cancerogenic); HTP-nc = Potential comparative Toxic Unit for humans
(not cancerogenic); SQP = Potential soil quality index
Disclaimer 1 – for the indicator IRP
This impact category deals mainly with the eventual impact of low dose ionizing radiation on human health of the nuclear fuel cycle. It
does not consider effects due to possible nuclear accidents, occupational exposure nor due to radioactive waste disposal in
underground facilities. Potential ionizing radiation from the soil, from radon and from some construction materials is also not measured
by this indicator.
Disclaimer 2 – for the indicators ADPE, ADPF, WDP, ETP-fw, HTP-c, HTP-nc, SQP
The results of this environmental impact indicator shall be used with care as the uncertainties on these results are high or as there is
limited experience with the indicator. This EPD was created using a software tool.
References
Standards (EAS), Radio Frequency Identification (RFID) and similar
applications.
CAN/CSA-22.2 No. 62368-1
CAN/CSA-22.2 No. 62368-1:2014, Audio/video, information and EN 55024+A1
communication technologyequipment — Part 1: Safety EN 55024:2010+A1:2015, Information technology equipment -
requirements. Immunity characteristics - Limits and methods of measurement.
Electromagnetic Compatibility Directive (EMC) EN 55032
Directive 2014/30/EU of the European Parliamant and of the EN 55032:2015, Electromagnetic compatibility of multimedia
Council of 26 February 2014 on the harmonisation of the laws equipment - Emission Requirements.
of the Member States relating to electromagnetic compatibility.
EN 60529
EN 15804+A2 EN 60529:2014, Degrees of protection provided by enclosures
EN 15804:2019+A2 (in press), Sustainability of construction (IP 20).
works — Environmental Product Declarations — Core rules for
the product category of construction products. EN 62368-1+A11
EN 62368-1:2014+A11:2017, Audio/video, information and
EN 300330 V2.1.1 communication technology equipment - Part 1: Safety
Short Range Devices (SRD) - Radio equipment in the requirements.
frequencyrange 9 kHz to 25 MHz and inductive loop systems in
the frequency range 9 kHz to 30 MHz - Harmonised Standard ISO 14025
covering the essential requirements of article 3.2 of the DIN EN ISO 14025:2011-10, Environmental labels and
Directive 2014/53/EU. declarations — Type III environmental declarations —
Principles and procedures.
EN 301489-1 V2.2.1
ElectroMagnetic Compatibility (EMC) standard for radio Low Voltage Directive (LVD)
equipment and services - Part 1: Common technical Directive 2014/35/EU of the European Parliament and of the
requirements - Harmonised Standard covering the essential Council of 26 February 2014 on the harmonisation of the laws
requirements of article 3.1(b) of Directive 2014/53/EU and the of the Member States relating to the making available on the
essential requirements of article 6 of Directive 2014/30/EU. market of electrical equipment designed for use within certain
voltage limits.
EN 301489-3 V2.1.1
ElectroMagnetic Compatibility (EMC) standard for radio Radio Equipment Directive (RED)
equipment and services - Part 3: Specific conditions for Short- Directive 2014/53/EU of the European Parliament and of the
Range Devices (SRD) operating on frequencies between 9 kHz Council of 16 April 2014 on the harmonisation of the laws of the
and 246 GHz - Harmonised standard covering the essential Member States relating to the making available on the market
requirements of article 3.1(b) of Directive 2014/53/EU. of radio equipment and repealing Directive 1999/5/EC.
EN 50364 Registration, Evaluation, Authorisation and Restriction of
EN 50364:2010, Limitation of human exposure to Chemicals (REACH)
electromagnetic fields from devices operating in the frequency Regulation (EC) No 1907/2006 of the European Parliament and
range 0 Hz to 300 GHz, used in Electronic Article Surveillance of the Council on the Registration, Evaluation, Authorisation
6 Environmental Product Declaration - dormakaba - Access manager 92 30
and Restriction of Chemicals (REACH).
Gabi Software System and Database for Life Cycle Engineering
Restriction of Hazardous Substances (RoHS) 1992-2020 Version 10.0.0.71 University of Stuttgart Leinfelden-
Directive on the restriction of the use of certain hazardous Echterdingen
substances in electrical and electronic equipment (RoHS),
Directive (EU) No 2011/65. GaBi ts documentation
GaBi life cycle inventory data documentation (https://www.gabi-
UL 294 software.com/support/gabi/gabi-database-2020-lci-
UL 294:2013, Standard for Safety Access Control System Unit. documentation/).
UL 62368-1 LCA-tool dormakaba
UL 62368-1:2014, Standard for Audio/video, information and LCA tool, version 1.0.
communication technology equipment - Part 1: Safety Developed by Sphera Solutions GmbH.
requirements.
PCR Part A
Further References PCR – Part A:
Calculation Rules for the Life Cycle As-sessment and
IBU 2016 Requirements on the Project Re-port according to EN
Institut Bauen und Umwelt e.V.: General Instructions for the 15804+A2:2019, Version 1.0, Institut Bauen und Umwelt e.V.,
EPD programme of Institut Bauen und Umwelt e.V. Version www.ibu-epd.com.
2.0., Berlin: Institut Bauen und Umwelt e.V., 2021. www.ibu-
epd.com PCR Part B
PCR – Part B: Requirements on the EPD for Building Hardware
GaBi ts software product, version 1.3, Institut Bauen und Umwelt e.V., www.ibu-
Sphera Solutions GmbH epd.com, 2019.
7 Environmental Product Declaration - dormakaba - Access manager 92 30
Publisher
Institut Bauen und Umwelt e.V. +49 (0)30 3087748- 0
Hegelplatz 1 info@ibu-epd.com
10117 Berlin www.ibu-epd.com
Germany
Programme holder
Institut Bauen und Umwelt e.V. +49 (0)30 3087748- 0
Hegelplatz 1 info@ibu-epd.com
10117 Berlin www.ibu-epd.com
Germany
Author of the Life Cycle Assessment
Sphera Solutions GmbH +49 711 341817-0
Hauptstraße 111- 113 info@sphera.com
70771 Leinfelden-Echterdingen www.sphera.com
Germany
Owner of the Declaration
dormakaba International Holding GmbH +49 2333 793-0
DORMA Platz 1 info.de@dormakaba.com
58256 Ennepetal www.dormakaba.com
Germany
8 Environmental Product Declaration - dormakaba - Access manager 92 30
