ENVIRONMENTAL PRODUCT DECLARATION
as per ISO 14025 and EN 15804+A2
Owner of the Declaration VELUX Group
Publisher Institut Bauen und Umwelt e.V. (IBU)
Programme holder Institut Bauen und Umwelt e.V. (IBU)
Declaration number EPD-VEL-20230282-IBA2-EN
Issue date 21.08.2023
Valid to 20.08.2028
VELUX sun tunnel TCF for flat roof, flexible, polycarbonate dome
VELUX A/S
www.ibu-epd.com | https://epd-online.com
1. General Information
VELUX A/S VELUX sun tunnel TCF for flat roof, flexible,
polycarbonate dome
Programme holder Owner of the declaration
IBU – Institut Bauen und Umwelt e.V. VELUX Group
Hegelplatz 1 Ådalsvej 99
10117 Berlin 2970 Hørsholm
Germany Denmark
Declaration number Declared product / declared unit
EPD-VEL-20230282-IBA2-EN The declaration represents 1 piece of VELUX sun tunnel TCF for flat roof,
flexible, with an polycarrbonate dome.
This declaration is based on the product category rules: Scope:
Windows and doors , 01.08.2021 The declaration covers 100% of VELUX sun tunnel TCF for flat roof,
(PCR checked and approved by the SVR) flexible with a polycarbonate dome by Partizánske Building Components
SK, Slovakia.
Issue date The owner of the declaration shall be liable for the underlying information
and evidence; the IBU shall not be liable with respect to manufacturer
21.08.2023
information, life cycle assessment data and evidences.
The EPD was created according to the specifications of EN 15804+A2. In
Valid to
the following, the standard will be simplified as EN 15804.
20.08.2028
Verification
The standard EN 15804 serves as the core PCR
Independent verification of the declaration and data according to ISO
14025:2011
internally X externally
Dipl.-Ing. Hans Peters
(Chairman of Institut Bauen und Umwelt e.V.)
Florian Pronold Dr. Matthew Fishwick,
(Managing Director Institut Bauen und Umwelt e.V.) (Independent verifier)
1 Environmental Product Declaration - VELUX A/S - VELUX sun tunnel TCF for flat roof, flexible, polycarbonate dome
2. Product
Ethylene propylene diene monomer (EPDM) 3%
2.1 Product description/Product definition Stainless steel 2%
The VELUX flexible sun tunnel TCF is used for installation in Aluminium 1%
flat roofs which brings natural light into areas of the house Zinc alloy 1%
where a flat-roof window installation is either not possible or not Steel 1%
appropriate. The frame is made of white polyvinyl chloride Others 3%
(PVC). Sash and diffuser are made of acrylonitrile styrene
acrylate (ASA) plastic and the dome is made of transparent 1) 'This product/article/at least one partial article contains
plastic (polycarbonate). The tunnel is made of flexible reflective substances listed in the ECHA candidate list (date: 02.03.2022)
material. exceeding 0.1 percentage by mass:
• no
For the placing of the product on the market in the European
2) 'This product/article/at least one partial article contains other
Union/European Free Trade Association (EU/EFTA) (with the
carcinogenic, mutagenic, or toxic for reproduction (CMR)
exception of Switzerland) the Regulation (EU) No. 305/2011/
substances in categories 1A or 1B which are not on the ECHA
(CPR) applies. The product needs a declaration of performance
candidate list, exceeding 0.1 percentage by mass:
in accordance with the CPR taking into the European Technical
Assessment: ETA -13/0764 of 14/10/2015. The CE-marking for • not investigated with suppliers
the product takes into account the Declaration of Performance 3) 'Biocide products were added to this construction product or
in accordance with the CPR. For the application and use the it has been treated with biocide products (this then concerns a
respective national provisions apply. treated product as defined by the (EU) Regulation on Biocidal
Products No. 528/2012):
2.2 Application
• no
The sun tunnel for flat roofs can be installed in roof pitches
between 0° and 15°. The sun tunnel is applicable to flat roofing
materials. It can be integrated in roofing felt, roofing
Recycled content
membranes and in fully supported zinc or copper metal roofing.
2.3 Technical Data
The Declaration of Performance including relevant technical
specifications and test methods/test standards can be
downloaded from the website www.velux.com/ce.
Constructional data for TCF 0K14 1010
For other variants, see velux.com/ce The values stated in the table relate to the recycled material
Name Value Unit streams in VELUX production.
Reaction to fire E class
2.6 Manufacture
Resistance to upward load EN 1875 UL 1500 - A few components are produced/processed internally. The
Resistance to downward load EN 1873 UL 2500 - majority of products are bought from external suppliers and
Resistance to fire EN 13501-2 NPD - assembled into the final product.
External fire performance EN 13501-5 NPD -
The factory is ISO 9001 certified.
Water tightness EN 1873 9A -
Impact resistance - small hard body passed 2.7 Environment and health during manufacturing
NPD -
EN 1873 The factory is ISO14001 and ISO 45001 certified.
Impact resistance - large soft body EN 1873 NPD -
2.8 Product processing/Installation
Direct airborne sound insulation EN ISO 54 (-5;-
dB The sun tunnel is fitted directly to the roof with the screws
410-3 7)
supplied.
Thermal transmittance EN 1873 2.5 W/(m2K)
It is important that frame and roofing material are fitted
Luminous transmittance EN 410 NPD - according to the installation instructions. Distance from interior
Air permeability EN 1026 3 Class ceiling finish to the upper edge of battens (measured in the
Durability EN 1873 passed - centre of the tunnel): 0.2 - 0.9 m
Installation of a sun tunnel requires access to the attic and the
Performance data of the product in accordance with the
roof.
declaration of performance with respect to its essential
characteristics according to ETA -13/0764 of 14/10/2015. 2.9 Packaging
Performance data of the product, based on the harmonised
The packaging usually consists of:
standards, in accordance with the other provisions for
- cardboard
harmonization.
- paper
- polyethylene film
2.4 Delivery status
- polystyrene foam parts
The product is available in a diameter of 350 mm.
- steel
2.5 Base materials/Ancillary materials
The use of other packaging materials is possible, but
Composition of the sun tunnel TCF 0K14 1010:
insignificant in terms of quantity.
Polyvinyl chloride (PVC) 50%
Acrylonitrile Butadiene Styrene (ABS) 17%
The plastic packaging (polyethylene (PE) film, polystyrene foam
Polycarbonate 22%
2 Environmental Product Declaration - VELUX A/S - VELUX sun tunnel TCF for flat roof, flexible, polycarbonate dome
parts), paper and cardboard as well as steel can be recycled if
separated by type; alternatively, they - except steel - can be Water
incinerated. In the event of unforeseen exposure to water (flood), no
adverse effects on human health or the environment are to be
2.10 Condition of use expected.
The material composition of VELUX sun tunnels does not
change over their service life. Mechanical destruction
In the event of unforeseen mechanical destruction, VELUX sun
2.11 Environment and health during use
tunnels have to be replaced; apart from potential injuries from
VELUX sun tunnels do not contain any pollutants that could be sharp edges, no adverse effects on human health or the
released during use. environment are to be expected.
Environmental protection: According to current knowledge, 2.14 Re-use phase
hazards to water, air and soil cannot arise when the products VELUX sun tunnels can be dismantled manually without any
are used as intended. problems. The metal parts are usually recycled, and the plastic
parts are sent for thermal recycling for energy recovery.
Health protection: According to current knowledge, no health Tempered glass can be recycled.
hazards or impairments are to be expected.
2.15 Disposal
2.12 Reference service life VELUX sun tunnels are mostly inert and can be disposed of in
It is not possible to calculate the reference service life an appropriate landfill. However, due to the value of the
according to ISO 15686. The service life based on a materials or the carbon content of the plastic parts, recycling or
manufacturer's declaration is 30 years. The corresponding energy recovery is preferable and common.
utilization scenario is declared in 4.
Waste code according to the European Waste List (Regulation
2.13 Extraordinary effects
on the European Waste List):
Fire 17 02 02 glass
Fire performance according to EN 13501-1 17 02 03 plastics
17 04 14 mixed metals
Name Value
Building material class B 2.16 Further information
Burning droplets s1 Further documentation on the products, technical data sheets,
Smoke gas development d0 BIM files, etc. can be found at:
www.velux.com
3. LCA: Calculation rules
material (plastics) is assumed to be thermally treated in a
3.1 Declared Unit municipal waste incineration plant with an efficiency R1 < 0.6
The declared unit is 1 piece of VELUX sun tunnel TCF for flat (according to the ecoinvent v3.8 (cut-off) dataset used); the
roof, flexible, with an polycarbonate dome (TCF 0K14 1010) for recovered energy is declared as exported energy. Metals,
a diameter of 350 mm. paper and cardboard are recycled; it is assumed that these
Declared unit fractions reach the end-of-waste state after having been sorted
and transported (as a conservative choice) to a recycler. No
Name Value Unit
packaging waste is landfilled.
Declared unit 1 piece
Area 0.1225 m² Modules B1 to B7 are not relevant for the product under
Mass reference 9.34 kg/pce consideration or no significant environmental impacts occur.
Module C1 includes manual dismantling, with no significant
3.2 System boundary environmental impact.
Type of EPD: Cradle to gate with options, with modules C1 –
Module C2 comprises the transport of the dismantled VELUX
C4, and module D (A1-A3, C, D and additional modules)
sun tunnel to a sorting plant and then to a waste incineration
plant for the thermally treated plastic fraction.
The production of VELUX sun tunnels (modules A1-A3)
includes raw material extraction, energy generation, waste
Modules C3/C4: given the complexity of the inventoried
treatment and all transports up to the factory gate. In
products, a mixed end-of-life scenario is modelled, allowing the
accordance with COUNCIL REGULATION (EU) No 333/2011,
different materials to follow their most likely path.
secondary metals are modelled as part of the product system
As a rule of thumb, metals are recycled and plastics are
from the moment they are available as unmixed scrap.
incinerated (also due to the very limited data available on
Waste or secondary fuels are not used for production.
plastics recycling and its benefits); for recycled metals, it is
assumed that these fractions reach the end-of-waste state after
Module A4 is not declared due to large variances in transport
having been sorted and transported to a recycler. The
distances between the production site and the construction site,
combustible material (plastics, etc.) is assumed to be thermally
where the product is installed.
treated in a municipal waste incineration plant.
Module A5: The products are delivered to the construction site
Module D includes the benefits and burdens associated with
ready to be installed. Manual installation is assumed; electricity
recycling metals beyond the system boundary, resulting from
consumption related to electric drilling machines, screwdrivers,
the treatment of recycled materials from the point of end-of-
etc. is considered to be negligible. The combustible packaging
3 Environmental Product Declaration - VELUX A/S - VELUX sun tunnel TCF for flat roof, flexible, polycarbonate dome
waste to the point of substitution (as loads) and substitution of good.
primary resources (as benefits).
It also includes the benefits and burdens associated with 3.7 Period under review
energy recovery from plastic waste in a municipal waste The LCA data represents the production conditions for the year
incineration plant, as modelled in Module C3. 2021.
In Module D, only net flows of metals leaving the product
3.8 Geographic Representativeness
system are considered.
Land or region, in which the declared product system is
manufactured, used or handled at the end of the product´s
lifespan: Europe
3.3 Estimates and assumptions
3.9 Allocation
No further assumptions and estimates relevant to the result had
No co-products are generated during the production of the
to be made beyond the points made in this chapter 3 and
VELUX products. Sorted production scrap of the different
chapter 4.
metals, notably aluminium, is considered a secondary material
3.4 Cut-off criteria with no economic value (so no burdens allocated) and
No data available from the company survey was neglected. considered in the quantification of net flows leaving the product
These include, among other things, material use, energy system. This approach is chosen to ensure a coherent
demand (heat, electricity), packaging materials of raw materials quantification of net flows entering module D.
(in so far as they are generated as waste) and product
packaging, consumables in production, waste treatment and No processes were modelled as part of the foreground model
the transport of all inputs and outputs. that would have required an allocation of multi-input processes.
With this approach, mass and energy flows below 1% were also Background datasets on municipal waste incineration plants
accounted for, up to a total of 5%. No processes were were taken from ecoinvent v3.8 (cut-off) without any
neglected that would have been known to the project managers modification.
and would have contributed significantly to the indicators of the
impact assessment. Allocation of reuse, recycling and recovery was avoided by the
cut-off approach in the foreground model in line with DIN EN
3.5 Background data 15804.
Ecoinvent v3.8 (cut-off) (2021) is used as the background
3.10 Comparability
database.
Basically, a comparison or an evaluation of EPD data is only
3.6 Data quality possible if all the data sets to be compared were created
The foreground data are based on extensive and detailed data according to EN 15804 and the building context, respectively
collection at the production site. The foreground data could be the product-specific characteristics of performance, are taken
fully linked with corresponding data records from the into account.
background database ecoinvent v3.8 (cut-off). Ecoinvent v3.8 (cut-off) has been used as the background
The background data was updated in 2021. Thus, the quality of database.
the foreground and background data can be rated as very
4. LCA: Scenarios and additional technical information
Metals and cardboard are recycled; it is assumed that these
Characteristic product properties of biogenic carbon fractions reach the end-of-waste state after having been sorted
Information on describing the biogenic carbon content at and transported (as a conservative choice) to a recycler over
factory gate 150 km with a lorry with a payload of 16-32 metric tons,
EURO6.
Name ValueUnit
No packaging waste is landfilled.
kg
Biogenic carbon content in product - The use of multi-way pallets is not taken into account as
C
packaging material.
Biogenic carbon content in accompanying kg
< 5%
packaging C Reference service life
Note: 1 kg of biogenic carbon is equivalent to 44/12 kg of CO .
2
Module A5
The products are delivered to the construction site ready to be
installed. Manual installation is assumed, and electricity
consumption related to electric drilling machines, screwdrivers,
etc. is considered to be negligible.
The combustible packaging material (plastics) is assumed to be
transported 50 km with a lorry with a payload of 16-32 metric
tons, EURO6 to an incineration plant with an efficiency R1 < 0.6
(according to the ecoinvent v3.8 (cut-off) dataset used); the
recovered energy is declared as exported energy; for its
quantification, an efficiency of 25.6% is assumed for the
production of heat and 13.0% for the production of electricity
(always referring to the lower heating value of the waste).
4 Environmental Product Declaration - VELUX A/S - VELUX sun tunnel TCF for flat roof, flexible, polycarbonate dome
Name Value Unit of-life scenario is modelled, allowing the different materials to
follow their most likely path.
Reference service life
It should also be noted that the deconstruction and waste
according to 30 a
treatment scenario can vary a lot, depending on the actual
manufacturer's declaration
situation. Thus, a generic end-of-life scenario is assumed.
The product has passed
Declared product As a rule of thumb, metals are recycled, plastics are incinerated
internal quality controls and
properties (at the gate) and - (also due to the very limited availability on plastics recycling
complies with EN 1873 for CE
finishes and its benefits).
marking
The combustible material (mainly plastics) is assumed to be
An assumed quality of
Carried out in accordance transported 50 km with a lorry with a payload of 16-32 metric
work, when installed in
with the manufacturer's - tons, EURO6 to an incineration plant.
accordance with the
instructions. Metals are recycled; it is assumed that these fractions reach the
manufacturer’s instructions
end-of-waste state after having been sorted and transported to
Design application a recycler over 150 km with a lorry with a payload of 16-32
parameters (if instructed by metric tons, EURO6.
Installation according to
the manufacturer),
assembly instructions and -
including the references to Module C3
state of the art.
the appropriate practices A consumption of 0.03 kWh/kg of electricity for shredding and
and application codes sorting and 0.437 MJ/kg of diesel fuel for internal logistics are
Outdoor environment, (for The declared products are taken into account to disassemble the product. The recovered
outdoor applications), e.g. intended for installation material leaves the product system as 'materials for recycling'.
weathering, pollutants, UV outside the building: They are The net amounts of the metals leaving the product system are
-
and wind exposure, therefore designed to considered as 'use of secondary material' in Module D.
building orientation, withstand outdoor conditions
shading, temperature throughout their service life. Module C4
Indoor environment (for As stated above, it is assumed that 100% of the plastic parts
indoor applications), e.g. The declared products are are treated in a waste incineration plant with an efficiency R1
temperature, moisture, not intended for installation - < 0.6 (according to the ecoinvent v3.8 (cut-off) dataset used);
chemical exposure inside a building. 25.57% of the lower heating value of the plastic parts are
recovered as heat and 13.0% as electricity. Recovered energy
Usage conditions, e.g. Standard use in any type of
is reported as 'exported energy' and considered in Module D.
frequency of use, building, i.e. opening/closing -
mechanical exposure as often as necessary.
Module D
The declared products are
Module D contains the benefits and loads beyond the system
Maintenance e.g. required designed for a reference life
boundary related to the recycling of metals, which result from
frequency, type and quality of 30 years. They are
- the treatment of recycled materials from the point of end-of-
and replacement of maintained by cleaning water
waste status to the point of substitution (as loads) and the
components at the discretion of the
substitution of primary resources (as benefits).
building occupants.
It also includes the benefits and loads related to the energy
Module C1 recovery from plastic wastes in a MWIP as modelled in
Manual de-installation is assumed, electricity consumption Modules A3, A5 and C3.
related to electric screw drivers, etc. is considered to be Due to a lack of data for plastics from de-construction activities,
negligible. Thus, no environmental impacts are declared in the substitution potential of recycled plastics is not taken into
module C1. account.
Only net flows leaving the product system are considered in
Module C2 module D.
Given the complexity of the inventoried products, a mixed end-
5 Environmental Product Declaration - VELUX A/S - VELUX sun tunnel TCF for flat roof, flexible, polycarbonate dome
5. LCA: Results
DESCRIPTION OF THE SYSTEM BOUNDARY (X = INCLUDED IN LCA; MND = MODULE OR INDICATOR NOT DECLARED; MNR
= MODULE NOT RELEVANT)
Benefits and
Construction loads beyond
Product stage Use stage End of life stage
process stage the system
boundaries
la ire ta m w a Ry lp p u s tro p s n a rT g n iru tc a fu n a M e h t m o rf tro p s n a rTe tis e h t o t e ta g y lb m e s s A e s U e c n a n e tn ia M ria p e R tn e m e c a lp e R tn e m h s ib ru fe R y g re n e la n o ita re p Oe s u re ta w la n o ita re p Oe s u n o itc u rts n o c -e Dn o itilo m e d tro p s n a rT g n is s e c o rp e ts a W la s o p s iD -e s u e R-y re v o c e R-g n ilc y c e Rla itn e to p
A1 A2 A3 A4 A5 B1 B2 B3 B4 B5 B6 B7 C1 C2 C3 C4 D
X X X MND X MND MND MNR MNR MNR MND MND X X X X X
RESULTS OF THE LCA - ENVIRONMENTAL IMPACT according to EN 15804+A2: 1 piece VELUX sun tunnel TCF 0K14 1010 for
flat roof, flexible, polycarbonate dome
Parameter Unit A1-A3 A5 C1 C2 C3 C4 D
GWP-total kg CO 2 eq 5.37E+01 2.73E+00 0 7.34E-02 2.65E-01 2.06E+01 -1.24E+01
GWP-fossil kg CO 2 eq 5.56E+01 7.66E-01 0 7.34E-02 2.05E-01 2.06E+01 -1.24E+01
GWP-biogenic kg CO 2 eq -2.03E+00 1.97E+00 0 0 5.91E-02 0 0
GWP-luluc kg CO 2 eq 6.1E-02 2.43E-05 0 2.98E-05 2.29E-04 5.33E-03 -1.66E-02
ODP kg CFC11 eq 1E-05 1.37E-08 0 1.72E-08 1.26E-08 1.81E-06 -8.54E-07
AP mol H+ eq 2.36E-01 3.99E-04 0 4.16E-04 7.84E-04 2.08E-02 -3.59E-02
EP-freshwater kg P eq 1.45E-03 4.76E-07 0 5.4E-07 2.66E-05 1.58E-04 -9.08E-04
EP-marine kg N eq 4.39E-02 1.52E-04 0 1.5E-04 2.51E-04 4.82E-03 -6.13E-03
EP-terrestrial mol N eq 4.57E-01 1.68E-03 0 1.65E-03 2.85E-03 5.3E-02 -7.07E-02
kg NMVOC
POCP 1.57E-01 4.71E-04 0 4.7E-04 7.61E-04 1.41E-02 -2.11E-02
eq
ADPE kg Sb eq 5.46E-04 2.03E-07 0 2.46E-07 3.58E-07 4.22E-05 -4.29E-05
ADPF MJ 8.71E+02 8.98E-01 0 1.13E+00 2.84E+00 4.03E+01 -1.69E+02
m3 world eq
WDP 2.38E+01 3.9E-03 0 3.71E-03 7.07E-03 3.01E+00 -8.22E-01
deprived
GWP = Global warming potential; ODP = Depletion potential of the stratospheric ozone layer; AP = Acidification potential of land and water; EP =
Eutrophication potential; POCP = Formation potential of tropospheric ozone photochemical oxidants; ADPE = Abiotic depletion potential for non-fossil
resources; ADPF = Abiotic depletion potential for fossil resources; WDP = Water (user) deprivation potential)
RESULTS OF THE LCA - INDICATORS TO DESCRIBE RESOURCE USE according to EN 15804+A2: 1 piece VELUX sun tunnel
TCF 0K14 1010 for flat roof, flexible, polycarbonate dome
Parameter Unit A1-A3 A5 C1 C2 C3 C4 D
PERE MJ 2.25E+01 2.26E+01 0 1.6E-02 3.59E-01 4.56E+00 -1.59E+01
PERM MJ 2.34E+01 -2.26E+01 0 0 -7.61E-01 0 0
PERT MJ 4.59E+01 1.41E-02 0 1.6E-02 -4.03E-01 4.56E+00 -1.59E+01
PENRE MJ 6.33E+02 1.03E+01 0 1.13E+00 2.27E-06 2.69E+02 -1.71E+02
PENRM MJ 2.38E+02 -9.37E+00 0 0 0 -2.28E+02 0
PENRT MJ 8.71E+02 8.98E-01 0 1.13E+00 2.27E-06 4.04E+01 -1.71E+02
SM kg 4.49E-01 0 0 0 0 0 1.37E+00
RSF MJ 0 0 0 0 0 0 0
NRSF MJ 0 0 0 0 0 0 0
FW m3 5.5E-01 2.13E-04 0 1.23E-04 6.78E-04 7.98E-02 -4.13E-02
PERE = Use of renewable primary energy excluding renewable primary energy resources used as raw materials; PERM = Use of renewable primary
energy resources used as raw materials; PERT = Total use of renewable primary energy resources; PENRE = Use of non-renewable primary energy
excluding non-renewable primary energy resources used as raw materials; PENRM = Use of non-renewable primary energy resources used as raw
materials; PENRT = Total use of non-renewable primary energy resources; SM = Use of secondary material; RSF = Use of renewable secondary fuels;
NRSF = Use of non-renewable secondary fuels; FW = Use of net fresh water
RESULTS OF THE LCA – WASTE CATEGORIES AND OUTPUT FLOWS according to EN 15804+A2:
1 piece VELUX sun tunnel TCF 0K14 1010 for flat roof, flexible, polycarbonate dome
Parameter Unit A1-A3 A5 C1 C2 C3 C4 D
HWD kg 1.87E-03 2.45E-06 0 2.88E-06 2.27E-06 7.1E-05 6.21E-05
NHWD kg 9.61E+00 6.88E-02 0 7.57E-02 1.16E-02 1.18E+00 -2.26E+00
RWD kg 2.31E-03 1.27E-05 0 1.63E-05 2.57E-05 3E-04 -6.98E-04
CRU kg 0 0 0 0 0 0 0
MFR kg 1.12E+00 1.35E+00 0 0 8.01E-01 0 0
MER kg 0 0 0 0 0 0 0
EEE MJ 4.32E-01 1.22E+00 0 0 0 2.97E+01 0
6 Environmental Product Declaration - VELUX A/S - VELUX sun tunnel TCF for flat roof, flexible, polycarbonate dome
EET MJ 8.49E-01 2.39E+00 0 0 0 5.84E+01 0
HWD = Hazardous waste disposed; NHWD = Non-hazardous waste disposed; RWD = Radioactive waste disposed; CRU = Components for re-use;
MFR = Materials for recycling; MER = Materials for energy recovery; EEE = Exported electrical energy; EET = Exported thermal energy
RESULTS OF THE LCA – additional impact categories according to EN 15804+A2-optional:
1 piece VELUX sun tunnel TCF 0K14 1010 for flat roof, flexible, polycarbonate dome
Parameter Unit A1-A3 A5 C1 C2 C3 C4 D
Disease
PM 3.75E-06 6.84E-09 0 8.1E-09 1.24E-08 1.65E-07 -3.43E-07
incidence
IR kBq U235 eq 1.23E+00 3.85E-03 0 4.9E-03 9.85E-03 1.74E-01 -2.92E-01
ETP-fw CTUe 1.1E+03 3.36E+00 0 8.94E-01 1.67E+00 7.61E+02 -1.38E+02
HTP-c CTUh 8.66E-08 1.27E-10 0 3.57E-11 4.51E-11 5.81E-09 -1.94E-08
HTP-nc CTUh 9.05E-07 1.63E-09 0 1.03E-09 1.47E-09 1.98E-07 -1.11E-07
SQP SQP 1.74E+02 7.53E-01 0 9.63E-01 3.83E-01 1.17E+01 -1.9E+01
PM = Potential incidence of disease due to PM emissions; IR = Potential Human exposure efficiency relative to U235; ETP-fw = Potential comparative
Toxic Unit for ecosystems; HTP-c = Potential comparative Toxic Unit for humans (cancerogenic); HTP-nc = Potential comparative Toxic Unit for humans
(not cancerogenic); SQP = Potential soil quality index
Disclaimer 1 – for the indicator “Potential Human exposure efficiency relative to U235”.This impact category deals mainly with the
eventual impact of low dose ionizing radiation on human health of the nuclear fuel cycle. It does not consider effects due to possible
nuclear accidents, occupational exposure or radioactive waste disposal in underground facilities. Potential ionizing radiation from the
soil, radon and from some construction materials is also not measured by this indicator.
Disclaimer 2 – for the indicators “abiotic depletion potential for non-fossil resources”, “abiotic depletion potential for fossil resources”,
“water (user) deprivation potential, deprivation-weighted water consumption”, “potential comparative toxic unit for ecosystems”,
“potential comparative toxic unit for humans – cancerogenic”, “Potential comparative toxic unit for humans - not cancerogenic”,
“potential soil quality index”. The results of this environmental impact indicator shall be used with care as the uncertainties on these
results are high as there is limited experience with the indicator.
6. LCA: Interpretation
Figure 1 illustrates the relative contributions of the different A1-A3 = 100%).
modules along the life cycle of the declared products (Modules
significance depending on the indicator and fluctuate between -
Figure 1: Relative environmental impacts of the different 5% and -60%.
life cycle stages for the VELUX sun tunnel TCF 0K14 1010 The use of renewable primary energy is mainly caused by the
(Modules A1-A3 = 10%) share of renewable energy in the electricity mix, thus the
production stage is the main driver of this impact category; the
The LCA is dominated by the manufacture of the product same holds also for the use of non-renewable primary energy.
(modules A1-A3); further relevant contributions come only from Material use of primary energy is negligible and related to
the incineration of the plastic waste in module C4. plastic parts of the product and packaging material. The
The benefits and burdens outside the product system vary in material use of primary energy is transferred to its energy use
7 Environmental Product Declaration - VELUX A/S - VELUX sun tunnel TCF for flat roof, flexible, polycarbonate dome
when the materials containing primary energy are incinerated ores and related to the disposal of road infrastructure;
with energy recovery. hazardous and radioactive waste are mainly caused by the
Non-hazardous waste as the quantitatively most relevant waste nuclear power in the electricity mix.
flows is mainly caused during mining andprocessing of metal
7. Requisite evidence
7.1 Formaldehyde standard.
Not tested based on applicable product standard.
7.2 MDI 7.4. Fire gas toxicity
Not tested based on applicable product standard. Not tested based on applicable product standard.
7.3 Checking of pre-treatment of substances used 7.5 VOC emissions
according to AltholzVO Not tested based on applicable product standard.
Not applicable; not tested based on applicable product
8. References
Product category rules of IBU ISO 14001
DIN EN ISO 14001:2015: Environmental management
IBU (2021) systems - Requirements with guidance for use.
IBU (2021): General Instructions for the EPD Programme of the
Institut Bauen und Umwelt e.V.. Version 2.0, Institut Bauen und ISO 45001
Umwelt e.V., Berlin ISO 45001:2018-03, Occupational health and safety
management systems - Requirements with guidance for use.
IBU (2022)
IBU (2022): Product category rules for building-related products EN 1873
and service, PCR Part A: Calculation rules for the life cycle DIN EN 1873:2005, Prefabricated accessories for roofing -
assessment and requirements for the project report. Version Individual rooflights of plastics - product specification and test
2.2., Institut Bauen und Umwelt e.V., Berlin. methods.
IBU (2023) ECHA candidate list
IBU (2023): PCR Guidance-Texts for Building-Related Products The Candidate List of Substances of Very High Concern for
and Services, PCR Part B: Requirements on the EPD for Authorisation, European Chemicals Agency, Helsinki.
windows and doors. Version 2023/04, Institut Bauen und
Umwelt e.V., Berlin. Regulation on biocidal products
REGULATION (EU) No 528/2012 OF THE EUROPEAN
Standards and legal documents PARLIAMENT AND OF THE COUNCIL of 22 May 2012
concerning the making available on the market and use of
EN 15804 biocidal products.
DIN EN 15804+A2:2022-3, Sustainability of construction
works - Environmental product declarations - Core rules for the Regulation (EU) Nr. 305/2011(CPR)
product category construction products. German version EN REGULATION (EU) No 305/2011 OF THE EUROPEAN
15804:2012+A2:2019 + AC:2021 PARLIAMENT AND OF THE COUNCIL of 9 March 2011 laying
down harmonised conditions for the marketing of construction
ISO 14025 products and repealing Council Directive 89/106/EEC.
DIN EN ISO 14025:2006-07, Environmental labels and
declarations - Type III Environmental declarations - Principles COUNCIL REGULATION (EU) No 333/2011
and procedures. COUNCIL REGULATION (EU) No 333/2011 of 31 March 2011
establishing criteria determining when certain types of scrap
ISO 14044 metal cease to be waste under Directive 2008/98/EC of the
DIN EN ISO 14044:2006-07, Environmental management - Life European Parliament and of the Council.
cycle assessment - Requirements and guidance (ISO
14044:2006); German and English versions EN ISO European Waste List (Waste index)
14044:2006. http://www.gesetze-im-internet.de/avv/anlage.htm
ISO 9001 Additional references
DIN EN ISO 9001:2015, Quality management systems -
Requirements. ecoinvent 3.8
ecoinvent 3.8, LCA database, 12/2021. Ecoinvent centre,
Zürich.
8 Environmental Product Declaration - VELUX A/S - VELUX sun tunnel TCF for flat roof, flexible, polycarbonate dome
Publisher
Institut Bauen und Umwelt e.V. +49 (0)30 3087748- 0
Hegelplatz 1 info@ibu-epd.com
10117 Berlin www.ibu-epd.com
Germany
Programme holder
Institut Bauen und Umwelt e.V. +49 (0)30 3087748- 0
Hegelplatz 1 info@ibu-epd.com
10117 Berlin www.ibu-epd.com
Germany
Author of the Life Cycle Assessment
Dr. Frank Werner - Umwelt & Entwicklung + 41 (0)44 241 39 06
Kammelenbergstrasse 30 frank@frankwerner.ch
9011 St. Gallen http://www.frankwerner.ch/
Switzerland
Owner of the Declaration
VELUX Group +4545164726
Ådalsvej 99 jakob.roerbech@velux.com
2970 Hørsholm www.velux.com
Denmark
9 Environmental Product Declaration - VELUX A/S - VELUX sun tunnel TCF for flat roof, flexible, polycarbonate dome
