ENVIRONMENTAL
as per ISO 14025 and EN 15804+A2
Owner of the Declaration Interface®
Programme holder Institut Bauen und Umwelt e.V. (IBU)
Publisher Institut Bauen und Umwelt e.V. (IBU)
Declaration number EPD-INT-20220226-CBB1-EN
Issue date 17.02.2023
Valid to 16.02.2028
Modular carpet tiles with Sone acoustic felt covered
CQuest Bio heavy backing
pile material: solution-dyed polyamide 6 yarn 100% recycled,
with a maximum total pile weight of 1500 g/m2
Interface®
www.ibu-epd.com | https://epd-online.com
Umwelt Produktdeklaration Name des Herstellers – Name des Produkts
General Information
Interface® Modular carpet tiles with Sone
acoustic felt covered CQuest Bio
heavy backing
pile material: solution-dyed polyamide
6 yarn 100% recycled with a maximum
total pile weight of 1500 g/m2
Programme holder Owner of the declaration
IBU – Institut Bauen und Umwelt e.V. Interface Europe Manufacturing BV
Hegelplatz 1 Industrielaan 15
10117 Berlin 3925 ZG Scherpenzeel
Germany The Netherlands
Declaration number Declared product / declared unit
EPD-INT-20220226-CBB1-EN 1 m² tufted modular carpet tiles with Sone acoustic felt
covered CQuest Bio (CQB) heavy backing and a pile
material of PA 6 with 100% recycled content
This declaration is based on the product Scope:
category rules: The manufacturer declaration applies to tufted carpet
Floor coverings, 02/2018 tiles with a Sone polyester felt covered CQuest Bio
(PCR checked and approved by the SVR) backing, a pile material of 100% recycled PA 6 with a
maximum total pile weight of 1500 g/m2. The products
are tufted in Scherpenzeel, the Netherlands, or in
Issue date
Craigavon, Ireland. Backing is applied in
17.02.2023
Scherpenzeel, Netherlands.
LCA results for products with a maximum total pile
Valid to weight of 535 g/m2 can be taken from the
16.02.2028 corresponding tables of the annexe. Specific data for
every product within the declared group of products in
relation to its total pile weight can be calculated by
using equation 1 given in the annexe (see annexe
chapter: 'General Information on the annexe'). The
declaration is only valid in conjunction with a valid
GUT-PRODIS license of the product.
The owner of the declaration shall be liable for the
underlying information and evidence; the IBU shall not
be liable with respect to manufacturer information, life
cycle assessment data and evidences.
The EPD was created according to the specifications
of EN 15804+A2. In the following, the standard will be
simplified as EN 15804.
Verification
The standard EN 15804 serves as the core PCR
Independent verification of the declaration and data
according to ISO 14025:2011
Dipl. Ing. Hans Peters internally x externally
(chairman of Institut Bauen und Umwelt e.V.)
Dr. Alexander Röder Prof. Dr. Birgit Grahl
(Managing Director Institut Bauen und Umwelt e.V.)) (Independent verifier)
Product
Product description/Product definition a recycled content of 98%. The total recycled content
The declaration applies to tufted carpet tiles having a of the carpet is 81%.
surface pile of 100% recycled solution dyed polyamide CQuest Bio backing system Sone: Backing compound
6 with a maximum total pile weight of 1500 g/m2. The based on renewable wood resin, containing a recycled
backing of the carpet consists of a CQuest Bio heavy filler, glass-fleece reinforcement and polyester
backing covered by a Sone acoustic polyester felt with covering fleece.
2 Environmental Product Declaration Interface – Tufted tiles, 100% rec. Polyamid 6, maximum total pile weight 1500 g/m2,
CQuest Bio backing, Sone acoustic cover
For the placing on the market of the specific product in PRODIS using the PRODIS registration number of the
the European Union/European Free Trade Association product (www.pro-dis.info) or on the manufacturer's
(EU/EFTA) (with the exception of Switzerland) technical information section.
Regulation (EU) No. 305/2011 Construction Product
Regulation (CPR) applies. The product needs a Base materials/Ancillary materials
Declaration of Performance (DoP) taking into
consideration EN 14041:2018-05, Resilient, textile and Name Value Unit
laminate floor coverings - Essential characteristics, and Polyamide 6 30.9 %
the CE-marking. The DoP of the product can be found Polyester 11.8 %
on the manufacturer's technical information section. Ethylene vinyl acetate (EVA) 4.9 %
For the application and use of the product the Wood resin 5.8 %
respective national provisions apply. Additives 1.6 %
Limestone 40.3 %
Application Aluminiumhydroxide 4.3 %
The use class of the specific product as defined in
Glass fiber 0.4 %
EN 1307 can be found in the Product Information
The specific product covered by the EPD contains
System (PRODIS) using the PRODIS registration
substances listed in the ECHA candidate list
number of the product.
(08.07.2021) exceeding 0.1 percentage by mass: no
This product contains other CMR substances in
Technical Data
categories 1A or 1B which are not on the candidate list
The performance data listed in the Declaration of
exceeding 0.1 percentage by mass: no
Performance (DoP) apply.
Biocide products were added to this construction
product or it has been treated with biocide products
Constructional data according to EN 1307
(this then concerns a treated product as defined by the
Name Value Unit
(EU) Ordinance on Biocide Products No. 528/2012): no
Modular carpet tiles, 50 cm x
Product Form - Aluminium hydroxide is used as fire retardant.
50 cm
Type of manufacture Tufted carpet -
Reference service life
Polyamide 6 from 100%
Yarn type - The service life of textile floor coverings strongly
recycled material
depends on the correct installation taking into account
Total carpet weight 4844 g/m2 the declared use classification and the adherence to
CQuest Bio backing with cleaning and maintenance instructions.
Secondary backing -
acoustic textile bottom Sone A calculation of the reference service life according to
ISO 15686 is not possible.
Alternatively, a reference service life of 15 years can
Performance data of the product in accordance with be assumed, during which the functional and visual
the declaration of performance with respect to its quality is guaranteed (In accordance with the warranty
essential characteristics according to EN 14041: 2018- of the manufacturer). The technical service life can be
05, Resilient, textile and laminate floor coverings - significantly longer.
Essential characteristics.
Additional product properties in accordance with EN
1307 can be found on the Product Information System
LCA: Calculation rules
Declared Unit
The indicated values refer to a virtual reference System boundary
product with the max. total pile weight and the max.
total weight. Type of EPD: Cradle-to-gate with options
Name Value Unit System boundaries of modules A, B, C, D:
Declared unit 1 m2 Modules C3, C4 and D are indicated separately for
Grammage (declared virtual product) 4.844 kg/m2 three end-of-life scenarios:
Total thickness (heaviest real product) 9.6 mm 1 - landfill disposal
Gross density (heaviest real product) 430 kg/m3 2 - municipal waste incineration
The declared unit refers to 1 m2 produced textile floor 3 - recovery in a cement plant
covering. The output of module A5 'Assembly' is 1 m2
installed textile floor covering. A1-A3 Production:
As the thickness of a virtual product cannot be Energy supply and production of the basic material,
calculated due to the fact that the total thickness does processing of secondary material, auxiliary material,
not depend on the total weight, the declared total transport of the material to the manufacturing site,
thickness and gross density refer to the heaviest real emissions, waste water treatment, packaging material
product. and waste processing up to the landfill disposal of
The layer thickness of the specific product covered by residual waste (except radioactive waste). Benefits for
the EPD can be found on the Product Information generated electricity and steam due to the incineration
System PRODIS using the PRODIS registration of production waste are aggregated.
number of the product (www.pro-dis.info) or on the Biogenic carbon that is stored in renewable material
manufacturer's technical information section. (wood resin, renewable additives,packaging paper) is
taken into account as well as the associated carbon
3 Environmental Product Declaration Interface – Tufted tiles, 100% rec. Polyamid 6, maximum total pile weight 1500 g/m2,
CQuest Bio backing, Sone acoustic cover
dioxide uptake from the air from which this biogenic The floor covering is de-constructed manually and no
carbon comes. additional environmental impact is caused.
A4 Transport: C2 Transport:
Transport of the packed textile floor covering Transport of the carpet waste to a landfill, to the
from factory gate to the place of installation. municipal waste incineration plant (MWI) or to the
waste collection facility for recycling.
A5 Installation:
Installation of the textile floor covering, processing of C3 Waste processing:
installation waste and packaging waste up to the C3-1: Landfill disposal needs no waste processing.
landfill disposal of residual waste (except radioactive C3-2: Impact from waste incineration (plant with R1 >
waste), the production of the amount of carpet that 0.6), generated electricity and steam are listed in the
occurs as installation waste including its transport to result table as exported energy.
the place of installation. C3-3: Collection of the carpet waste for recovery in the
Generated electricity and steam due to the incineration cement industry, waste processing (granulating),
of waste are listed in the result table as exported transport to the cement plant, emissions from the
energy. incineration.
Biogenic carbon that is stored in renewable materials
in installation waste and packaging paper is released C4 Disposal
as carbon dioxide emissions into the air at the end of C4-1: Impact from landfill disposal,
life in module A5. C4-2: The carpet waste leaves the system in module
Preparation of the floor and auxiliary materials C3-2,
(adhesives, fixing agents, PET connectors) are beyond C4-3: The pre-processed carpet waste leaves the
the system boundaries and not taken into account. system in module C3-3.
B1 Use: D Recycling potential:
Indoor emissions during the use stage. After the first Calculated benefits result from materials exclusive
year, no product-related Volatile Organic Compound secondary materials (net materials).
(VOC) emissions are relevant due to known VOC D-A5: Benefits for generated energy due
decay curves of the product. to incineration of packaging and installation waste
(incineration plant with R1 > 0.6),
B2 Maintenance: D-1: Assuming that the chemically bound renewable
Cleaning of the textile floor covering for a period of 1 materials in a landfill gas do not release landfill gas
year: within 100 years, no benefits due to landfill dosposal of
Vacuum cleaning – electricity supply carpet waste at the end-of-life are taken into account,
Wet cleaning – electricity, water consumption, D-2: Benefits for generated energy due to incineration
production of the cleaning agent, waste water of carpet waste at the end-of-life (incineration plant
treatment with R1 > 0.6),
The declared values in this module have to be D-3: Benefits for saved fossil energy and saved
multiplied by the assumed service life of the floor inorganic material due to recovery of the carpet in a
covering in the building in question. cement plant.
B3 - B5: Comparability
The modules are not relevant within the assumed Basically, a comparison or an evaluation of EPD data
reference service life of 15 years. is only possible if all the data sets to be compared
were created according to EN 15804 and the building
B6 - B7: context, respectively the product-specific
No energy and water input are required for the characteristics of performance, are taken into account.
operation of the carpet in the use stage. The modules
do not cause any environmental impact. Background data are taken from the GaBi database,
2022-1. Remaining data gaps are covered by the
C1 De-construction: ecoinvent 3.7 database, 2020.
LCA: Scenarios and additional technical information
Characteristic product properties
Information on biogenic Carbon
Transport to the construction site (A4)
Name Value Unit
Name Value Unit Litres of fuel (truck, EURO 0-6
0.0113 l/100km
Biogenic carbon content in mix)
0.26 kg C
product at factory gate Transport distance 700 km
Biogenic carbon content in Capacity utilisation (including
55 %
accompanying packaging at 0.05 kg C empty runs)
factory gate
1 kg biogenic Carbon is equivalent to 44/12 kg of CO Installation in the building (A5)
2
Name Value Unit
Material loss 0.145 kg
Polyethylene packaging waste and installation waste
are considered to be incinerated in a municipal waste
4 Environmental Product Declaration Interface – Tufted tiles, 100% rec. Polyamid 6, maximum total pile weight 1500 g/m2,
CQuest Bio backing, Sone acoustic cover
incineration plant. Cardboard packaging waste is going
to be recycled.
Preparation of the floor and auxiliaries (adhesives,
fixing agents, PET connectors etc.) are not taken into Name Value Unit
account. Collected as mixed construction
4.844 kg
waste (scenario 1 and 2)
Maintenance (B2) Collected separately (scenario 3) 4.844 kg
The values for cleaning refer to 1 m2 floor covering per Landfilling (scenario 1) 4.844 kg
year. Energy recovery (scenario 2) 4.844 kg
Depending on the application based on ISO 10874, the Energy recovery (scenario 3) 2.664 kg
technical service life recommended by the Recycling (scenario 3) 2.18 kg
manufacturer and the anticipated strain on the floor by
customers, the case-specific useful life can be Reuse, recovery and/or recycling potentials (D),
established. Based on this useful life the effects of relevant scenario information
module B2 need to be calculated in order to obtain the Recovery or recycling potentials due to the three end-
overall environmental impacts. of-life scenarios (module C) are indicated separately.
Recycling in the cement industry (scenario 3)
Name Value Unit The organic material of the carpet is used as an
Number
Maintenance cycle (vacuum cleaning) 208 alternative fuel in a cement kiln. It mainly substitutes
/year
for lignite (68.8%), hard coal (23.6%) and petrol coke
Maintenance cycle (wet cleaning) 1,5 Number (7.6%). The inorganic material is substantially
/year integrated into the cement clinker and substitutes for
Water consumption (wet cleaning) 0.004 m3 original material input. VDZ e.V.
Cleaning agent (wet cleaning) 0.09 kg
Electricity consumption 0.314 kWh
For further information on cleaning and maintenance
see www.interface.com
Service life
Name Value Unit
Life Span (according to
15 a
manufacturer's warranty)
Corresponds to
Declared product properties (at the
-
the gate) and finishes specifications of
EN 1307
An assumed quality of work, when Conforms to the
installed in accordance with the manufacturer's -
manufacturer’s instructions instructions
Use in areas
defined by the
Usage conditions, e.g. frequency
use class -
of use, mechanical exposure
according to EN
1307
Maintenance e.g. required According to the
frequency, type and quality and manufacturers -
replacement of components instructions
End of Life (C1-C4)
Three different end-of-life scenarios are declared and
the results are indicated separately in module C.
Each scenario is calculated as a 100% scenario.
Scenario 1: 100 % landfill disposal
Scenario 2: 100 % municipal waste incineration (MWI)
with R1 > 0.6
Scenario 3: 100 % recovery in the cement industry
If combinations of these scenarios have to be
calculated this should be done according to the
following scheme:
EOL-impact = x % impact (Scenario 1)
+ y % impact (Scenario 2)
+ z % impact (Scenario 3)
with x % + y % + z % = 100 %
5 Environmental Product Declaration Interface – Tufted tiles, 100% rec. Polyamid 6, maximum total pile weight 1500 g/m2,
CQuest Bio backing, Sone acoustic cover
LCA: Results
The LCA results refer to all declared products with a maximum total pile weight of 1500 g/m2. LCA results for
products with a maximum total pile weight of 535 g/m2 can be taken from the corresponding tables of the annexe.
Results for specific products with any other total pile weight can be calculated by using equation 1 given in the
annexe (see annexe chapter: 'General Information on the annexe'). The declared result figures in module B2 have
to be multiplied by the assumed service life (in years) of the floor covering in the building under consideration.
Information on non-relevant modules: Modules B3 - B7 are not relevant during the service life of the carpet.
Modules C1, C3/1, C4/2 and C4/3 cause no additional impact (see chapter "LCA: Calculation rules" in this
document). All these modules are declared and marked as 'modules not relevant/declared'. Module C2 represents
the transport for scenarios 1, 2 and 3. Column D represents benefits from module A5 assembly.
DESCRIPTION OF THE SYSTEM BOUNDARY (X = INCLUDED IN LCA; ND = MODULE OR INDICATOR NOT
DECLARED; MNR = MODULE NOT RELEVANT)
BENEFITS AND
CONSTRUCTI LOADS
PRODUCT STAGE ON PROCESS USE STAGE END OF LIFE STAGE BEYOND THE
STAGE SYSTEM
BOUNDARIES
6 Environmental Product Declaration Interface – Tufted tiles, 100% rec. Polyamid 6, maximum total pile weight 1500 g/m2,
CQuest Bio backing, Sone acoustic cover
lairetam
waR
ylppus tropsnarT
gnirutcafunaM
eht
morf
tropsnarT
etis
eht
ot
etag
ylbmessA esU
ecnanetniaM
riapeR
tnemecalpeR tnemhsibrufeR
ygrene
lanoitarepO esu
retaw
lanoitarepO esu
noitcurtsnoc-eD
noitilomed tropsnarT
gnissecorp
etsaW
lasopsiD -esueR -yrevoceR -gnilcyceR laitnetop
A1 A2 A3 A4 A5 B1 B2 B3 B4 B5 B6 B7 C1 C2 C3 C4 D
X X X X X X X MNR MNR MNR ND ND X X X X X
RESULTS OF THE LCA - ENVIRONMENTAL IMPACT according to EN 15804+A2: 1 m² floor covering
Core Indicator Unit A1-A3 A4 A5 B1 B2 C1 C2 C3/2 C3/3 C4/1 D D/1 D/2 D/3
GWP-total [kg CO2-Eq.] 4.64E+02.96E-1 4.26E-10.00E+04.16E-10.00E+01.64E-26.45E+06.52E+01.29E+0-2.14E-20.00E+0-2.59E-1-1.79E-1
GWP-fossil [kg CO2-Eq.] 5.95E+02.90E-1 4.10E-10.00E+02.15E-10.00E+01.61E-25.50E+05.57E+03.40E-1-2.13E-20.00E+0-2.57E-1-1.79E-1
-
GWP-biogenic [kg CO2-Eq.] 1.32E+03.75E-3 1.59E-20.00E+04.16E-30.00E+02.09E-4 9.49E-1 9.50E-1 9.48E-1-1.09E-40.00E+0-1.29E-3-3.18E-4
GWP-luluc [kg CO2-Eq.] 1.19E-2 1.64E-3 4.17E-40.00E+01.96E-10.00E+09.14E-5 2.29E-4 4.63E-4 1.67E-4-2.33E-60.00E+0-2.77E-5-8.81E-5
1.77E- 8.59E- 9.82E- 5.52E- 9.18E- 4.61E- -1.43E- -1.69E- -2.13E-
ODP [kg CFC11-Eq.] 2.86E-8 0.00E+03.42E-80.00E+0 0.00E+0
14 10 16 13 13 13 13 12 13
AP [mol H+-Eq.] 2.66E-2 1.75E-3 1.07E-30.00E+08.32E-40.00E+09.76E-5 7.01E-3 7.31E-3 1.02E-3-2.79E-50.00E+0-3.33E-4-7.10E-4
EP-freshwater [kg P-Eq.] 1.52E-4 8.80E-7 4.62E-60.00E+05.19E-60.00E+04.89E-8 8.47E-7 1.04E-6 6.41E-5-2.91E-80.00E+0-3.45E-7-1.95E-7
EP-marine [kg N-Eq.] 9.00E-3 8.61E-4 4.03E-40.00E+01.97E-40.00E+04.79E-5 3.48E-3 3.61E-3 2.25E-4-7.59E-60.00E+0-9.10E-5-2.10E-4
EP-terrestrial [mol N-Eq.] 8.44E-2 9.53E-3 4.02E-30.00E+02.83E-30.00E+05.30E-4 3.87E-2 4.02E-2 2.47E-3-8.13E-50.00E+0-9.75E-4-2.30E-3
POCP [kg NMVOC-Eq.]2.13E-2 1.63E-3 9.62E-4 4.18E-4 9.83E-40.00E+09.06E-5 8.91E-3 9.17E-3 7.24E-4-2.12E-50.00E+0-2.55E-4-6.25E-4
ADPE [kg Sb-Eq.] 2.59E-6 2.46E-8 7.94E-80.00E+02.30E-70.00E+01.37E-9 2.96E-8 3.98E-8 2.38E-8-3.20E-90.00E+0-3.81E-8-1.74E-8
- -
ADPF [MJ] 9.04E+13.94E+02.95E+00.00E+05.90E+00.00E+02.19E-13.60E+04.60E+04.87E+0-3.62E-10.00E+0
4.37E+01.94E+1
[m³ world-Eq
WDP 2.04E+12.64E-3 6.40E-10.00E+09.99E-20.00E+01.47E-4 8.23E-1 8.29E-1-3.64E-3-2.23E-30.00E+0-2.64E-2-2.54E-2
deprived]
GWP = Global warming potential; ODP = Depletion potential of the stratospheric ozone layer; AP = Acidification potential of land and water; EP =
Caption Eutrophication potential; POCP = Formation potential of tropospheric ozone photochemical oxidants; ADPE = Abiotic depletion potential for non-
fossil resources; ADPF = Abiotic depletion potential for fossil resources; WDP = Water (user) deprivation potential
RESULTS OF THE LCA - INDICATORS TO DESCRIBE RESOURCE USE according to EN 15804+A2: 1 m²
floor covering
Indicator Unit A1-A3 A4 A5 B1 B2 C1 C2 C3/2 C3/3 C4/1 D D/1 D/2 D/3
PERE [MJ] 8.87E+1 2.24E-1 3.36E+0 0.00E+0 3.69E+0 0.00E+0 1.25E-2 1.40E+1 1.43E+1 4.01E-1 -9.89E-2 0.00E+0 -1.17E+0-2.64E-1
PERM [MJ] 1.37E+1 0.00E+0 -2.60E-1 0.00E+0 0.00E+0 0.00E+0 0.00E+0 -1.34E+1-1.34E+1 0.00E+0 0.00E+0 0.00E+0 0.00E+0 0.00E+0
PERT [MJ] 1.02E+2 2.24E-1 3.10E+0 0.00E+0 3.69E+0 0.00E+0 1.25E-2 5.80E-1 8.61E-1 4.01E-1 -9.89E-2 0.00E+0 -1.17E+0-2.64E-1
PENRE [MJ] 8.27E+1 3.95E+0 3.35E+0 0.00E+0 5.90E+0 0.00E+0 2.20E-1 1.11E+1 1.21E+1 4.87E+0 -3.62E-1 0.00E+0 -4.37E+0-1.94E+1
PENRM [MJ] 7.87E+0 0.00E+0 -3.96E-1 0.00E+0 0.00E+0 0.00E+0 0.00E+0 -7.48E+0-7.48E+0 0.00E+0 0.00E+0 0.00E+0 0.00E+0 0.00E+0
PENRT [MJ] 9.05E+1 3.95E+0 2.96E+0 0.00E+0 5.90E+0 0.00E+0 2.20E-1 3.60E+0 4.60E+0 4.87E+0 -3.62E-1 0.00E+0 -4.37E+0-1.94E+1
SM [kg] 4.12E+0 0.00E+0 1.24E-1 0.00E+0 0.00E+0 0.00E+0 0.00E+0 0.00E+0 0.00E+0 0.00E+0 0.00E+0 0.00E+0 0.00E+0 1.50E-1
RSF [MJ] 0.00E+0 0.00E+0 0.00E+0 0.00E+0 0.00E+0 0.00E+0 0.00E+0 0.00E+0 0.00E+0 0.00E+0 0.00E+0 0.00E+0 0.00E+0 0.00E+0
NRSF [MJ] 0.00E+0 0.00E+0 0.00E+0 0.00E+0 0.00E+0 0.00E+0 0.00E+0 0.00E+0 0.00E+0 0.00E+0 0.00E+0 0.00E+0 0.00E+0 0.00E+0
FW [m³] 4.87E-1 2.53E-4 1.53E-2 0.00E+0 3.34E-3 0.00E+0 1.41E-5 1.95E-2 1.97E-2 5.71E-5 -9.45E-5 0.00E+0 -1.12E-3 -1.85E-3
PERE = Use of renewable primary energy excluding renewable primary energy resources used as raw materials; PERM = Use of
renewable primary energy resources used as raw materials; PERT = Total use of renewable primary energy resources; PENRE = Use of
non-renewable primary energy excluding non-renewable primary energy resources used as raw materials; PENRM = Use of non-
Caption
renewable primary energy resources used as raw materials; PENRT = Total use of non-renewable primary energy resources; SM = Use
of secondary material; RSF = Use of renewable secondary fuels; NRSF = Use of non-renewable secondary fuels; FW = Use of net fresh
water
RESULTS OF THE LCA – WASTE CATEGORIES AND OUTPUT FLOWS according to EN 15804+A2:
1 m² floor covering
Indicator Unit A1-A3 A4 A5 B1 B2 C1 C2 C3/2 C3/3 C4/1 D D/1 D/2 D/3
HWD [kg] 4.24E-3 1.89E-11 1.27E-4 0.00E+0 4.19E-5 0.00E+0 1.05E-125.56E-105.97E-107.51E-10-4.91E-110.00E+0-5.97E-10-1.62E-10
NHWD [kg] 7.03E-1 5.66E-4 5.45E-2 0.00E+0 7.30E-3 0.00E+0 3.15E-5 1.11E+0 1.11E+0 4.82E+0 -1.83E-4 0.00E+0 -2.18E-3 -9.83E-2
RWD [kg] 3.02E-3 4.86E-6 9.47E-5 0.00E+0 3.76E-4 0.00E+0 2.71E-7 1.25E-4 1.98E-4 5.99E-5 -2.84E-5 0.00E+0 -3.35E-4 -5.87E-5
CRU [kg] 0.00E+0 0.00E+0 0.00E+0 0.00E+0 0.00E+0 0.00E+0 0.00E+0 0.00E+0 0.00E+0 0.00E+0 0.00E+0 0.00E+0 0.00E+0 0.00E+0
MFR [kg] 0.00E+0 0.00E+0 1.21E-1 0.00E+0 0.00E+0 0.00E+0 0.00E+0 0.00E+0 1.25E+0 0.00E+0 0.00E+0 0.00E+0 0.00E+0 0.00E+0
MER [kg] 0.00E+0 0.00E+0 0.00E+0 0.00E+0 0.00E+0 0.00E+0 0.00E+0 0.00E+0 0.00E+0 0.00E+0 0.00E+0 0.00E+0 0.00E+0 0.00E+0
EEE [MJ] 0.00E+0 0.00E+0 3.33E-1 0.00E+0 0.00E+0 0.00E+0 0.00E+0 9.04E+0 0.00E+0 0.00E+0 0.00E+0 0.00E+0 0.00E+0 0.00E+0
EET [MJ] 0.00E+0 0.00E+0 6.09E-1 0.00E+0 0.00E+0 0.00E+0 0.00E+0 1.67E+1 7.94E+1 0.00E+0 0.00E+0 0.00E+0 0.00E+0 0.00E+0
HWD = Hazardous waste disposed; NHWD = Non-hazardous waste disposed; RWD = Radioactive waste disposed; CRU = Components
Caption for re-use; MFR = Materials for recycling; MER = Materials for energy recovery; EEE = Exported electrical energy; EET = Exported
thermal energy
RESULTS OF THE LCA – additional impact categories according to EN 15804+A2-optional:
1 m² floor covering
Indicator Unit A1-A3 A4 A5 B1 B2 C1 C2 C3/2 C3/3 C4/1 D D/1 D/2 D/3
[Disease -2.31E-
PM 2.07E-7 1.01E-8 7.38E-9 0.00E+0 6.84E-8 0.00E+05.64E-10 2.74E-8 2.93E-8 9.78E-9 0.00E+0 0.00E+0 -9.95E-9
Incidence] 10
[kBq U235-
IRP 4.90E-1 7.12E-4 1.53E-2 0.00E+0 6.78E-2 0.00E+0 3.96E-5 1.91E-2 3.14E-2 8.84E-3 -4.80E-3 0.00E+0 0.00E+0 -7.19E-3
Eq.]
ETP-fw [CTUe] 1.07E+2 2.73E+0 3.35E+0 3.60E-3 2.69E+0 0.00E+0 1.52E-1 1.67E+0 2.25E+0 4.77E+0 -7.91E-2 0.00E+0 0.00E+0-3.56E+0
-3.65E- -4.93E-
HTP-c [CTUh] 2.96E-9 5.53E-119.33E-110.00E+06.21E-100.00E+03.07E-128.39E-119.73E-112.14E-10 0.00E+0 0.00E+0
12 11
-1.40E-
HTP-nc [CTUh] 8.10E-8 3.28E-9 2.71E-9 2.60E-11 9.46E-9 0.00E+01.82E-10 5.44E-9 6.10E-9 1.79E-8 0.00E+0 0.00E+0 -3.13E-9
10
SQP [-] ND ND ND ND ND 0.00E+0 6.11E-2 6.49E-1 9.33E-1 2.84E-1 ND ND ND ND
PM = Potential incidence of disease due to PM emissions; IR = Potential Human exposure efficiency relative to U235; ETP-fw = Potential
Caption comparative Toxic Unit for ecosystems; HTP-c = Potential comparative Toxic Unit for humans (cancerogenic); HTP-nc = Potential
comparative Toxic Unit for humans (not cancerogenic); SQP = Potential soil quality index
No substantiated values can be given for the SQP indicator with the existing database.
The result figures given in module B2 refer to a period of 1 year because a reference service life is not declared.
They have to be multiplied by the assumed service life (in years) of the floor covering in the building under
consideration.
Disclaimer 1 – for the indicator “Potential Human exposure efficiency relative to U235”.
This impact category deals mainly with the eventual impact of low dose ionizingradiation on human health of the
nuclear fuel cycle. It does not consider effects due to possible nuclear accidents, occupational exposure nor due
to radioactive waste disposal in undergroundfacilities. Potential ionizing radiation from the soil, from radon and
from some construction materials is also not measured by this indicator.
Disclaimer 2 – for the indicators “abiotic depletion potential for non-fossil resources”, “abiotic depletion potential
for fossil resources”, “water (user) deprivation potential, deprivation-weighted water consumption”, “potential
comparative toxic unit for ecosystems”, “potential comparative toxic unit for humans – cancerogenic”, “Potential
comparative toxic unit for humans - not cancerogenic”, “potential soil quality index”.
The results of this environmental impact indicator shall be used with care as the uncertainties on these results are
high or as there is limited experienced with the indicator.
References
EN 1307 floor coverings – Environmental product declarations –
DIN EN 1307: 2014+A1:2016+A2:2018-05: Textile Product category rules
floor coverings - Classification
ISO 10874
EN 13501-1 DIN EN ISO 10874: 2012+A1:2021-04: Resilient,
DIN EN 13501-1:2019-05: Fire classification of textile and laminate floor coverings - Classification
construction products and building elements - Part 1:
Classification using data from reaction to fire tests ISO 14025
DIN EN /ISO 14025:2011-10/, Environmental labels
EN 14041 and declarations — Type III environmental
DIN EN 14041: 2018-05 and DIN EN 14041: 2008-05: declarations — Principles and procedures
Resilient, textile and laminate floor coverings -
Essential characteristics
ISO 14040
EN 15804 DIN EN ISO 14040:2006+A1:2020 Environmental
DIN EN 15804:2012+A2:2019 + AC:2021, management - Life cycle assessment - Principles and
Sustainability of construction works — Environmental framework
Product Declarations — Core rules for the product
category of construction products ISO 14044
DIN EN ISO 14044:2006+A1:2018+A2:2020
EN 16810 Environmental management - Life cycle assessment -
DIN EN 16810: 2017-08: Resilient, textile and laminate Requirements and guidelines
7 Environmental Product Declaration Interface – Tufted tiles, 100% rec. Polyamid 6, maximum total pile weight 1500 g/m2,
CQuest Bio backing, Sone acoustic cover
ISO 15686 GaBi database
ISO 15686: Buildings and constructed assets - GaBi Software-System and Database for Life Cycle
Service life planning Engineering, version 10.5 Sphera, Leinfelden-
ISO 15686-1: 2011-05: Part 1: General principles and Echterdingen, database version 2022-1
framework
ISO 15686-2: 2012-05: Part 2: Service life prediction PCR Part A
procedures Product Category Rules for Building-Related Products
ISO 15686-7: 2017-04: Part 7: Performance and Services Part A: Calculation Rules for the Life
evaluation for feedback of service life data Cycle Assessment and Requirements on the Project
from practice Report according to EN 15804+A2:2019, V1.2, Berlin:
ISO 15686-8: 2008-06: Part 8: Reference service life Institut Bauen und Umwelt e.V. (IBU), November 2021
and service-life estimation
PCR Part B
Regulation (EU) No. 305/2011 Product Category Rules for Building-Related Products
Regulation No. 305/2011 Construction Products and Services
Regulation (CPR) of the European Council and of the Part B: Requirements on the EPD for floor coverings,
European Parliament, April 2011 V1.2, Berlin: Institut Bauen und Umwelt e.V. (IBU),
February 2018
General Instructions for the IBU-EPD Program
General Instructions for the EPD-Program of the PRODIS
Institut Bauen und Umwelt e.V., The Preparation of Product Information System (PRODIS) of the
Environmental Product Declarations - EPDs, version European Carpet Industry, Gemeinschaft
2.0, Institut Bauen und Umwelt e.V., Berlin, January umweltfreundlicher Teppichboden e.V (GUT) and
2021, www.ibu-epd.de European Carpet and Rug Association
(ECRA), http://www.pro-dis.info
BNB, Nutzungsdauer von Bauteilen
Bewertungssystem Nachhaltiges Bauen (BNB), REACH
Nutzungsdauer von Bauteilen, Bundesministerium des Regulation (EC) No 1907/2006 of the European
Inneren, für Bau und Heimat, 24.02.2017 Parliament and of the Council of 18 December 2006
concerning the Registration, Evaluation, Authorisation
ECHA candidate list and Restriction of Chemicals (REACH), June 2017,
Candidate List of substances of very high concern last update: 08.07.2021
(SVHCs) for authorisation, 08.07.2021, European
Chemicals Agency (ECHA), Helsinki, Finland VDZ e.V.
Association of German Cement Works, Ed. Environ-
mental Data of the German Cement Industry 2020
ecoinvent
ecoinvent, Zurich, Switzerland, database version 3.7,
published September 2020
8 Environmental Product Declaration Interface – Tufted tiles, 100% rec. Polyamid 6, maximum total pile weight 1500 g/m2,
CQuest Bio backing, Sone acoustic cover
Publisher
Institut Bauen und Umwelt e.V. Tel +49 (0)30 3087748- 0
Hegelplatz 1 Fax +49 (0)30 3087748- 29
10117 Berlin Mail info@ibu-epd.com
Germany Web www.ibu-epd.com
Programme holder
Institut Bauen und Umwelt e.V. Tel +49 (0)30 - 3087748- 0
Hegelplatz 1 Fax +49 (0)30 – 3087748 - 29
10117 Berlin Mail info@ibu-epd.com
Germany Web www.ibu-epd.com
Author of the Life Cycle
Assessment Tel +49 (0)241 96843 410
Gemeinschaft umweltfreundlicher Fax +49 (0)241 96843 400
Teppichboden (GUT) e.V. Mail mail@gut-ev.de
Schönebergstraße 2 Web www.gut-ev.org
52068 Aachen
Germany
Owner of the Declaration
Interface Europe Manufacturing Tel +31 33 277 55 55
BV Fax +31 33 277 55 54
Industrielaan 15 Mail receptie@interface.com
3925ZG Scherpenzeel Web www.interface.com
Netherlands
