ENVIRONMENTAL PRODUCT DECLARATION
as per ISO 14025 and EN 15804+A2
Owner of the Declaration Knauf Integral KG
Publisher Institut Bauen und Umwelt e.V. (IBU)
Programme holder Institut Bauen und Umwelt e.V. (IBU)
Declaration number EPD-KNA-20220093-CAB1-EN
Issue date 26.06.2023
Valid to 25.06.2028
Knauf GIFAfloor DB 40 green
Knauf Integral KG
www.ibu-epd.com | https://epd-online.com
General Information
Knauf Integral KG Knauf GIFAfloor DB 40 green
Programme holder Owner of the declaration
IBU – Institut Bauen und Umwelt e.V. Knauf Integral KG
Hegelplatz 1 Am Bahnhof 16
10117 Berlin 74589 Satteldorf
Germany Germany
Declaration number Declared product / declared unit
EPD-KNA-20220093-CAB1-EN 1 m² of gypsum fibre panel Knauf GIFAfloor DB 40 green, 64.4 kg/m², 40
mm
This declaration is based on the product category rules: Scope:
Plasterboard, 01.08.2021 This EPD declares the environmental impacts of the gypsum fibre panels
(PCR checked and approved by the SVR) Knauf GIFAfloor DB 40 green, produced by Knauf Integral KG, plant
Satteldorf (Germany). It covers 100 % of the manufacture of Knauf
GIFAfloor DB 40 green in Satteldorf (D). The life cycle assessment is
Issue date based on production data for 2020.
The owner of the declaration shall be liable for the underlying information
26.06.2023
and evidence; the IBU shall not be liable with respect to manufacturer
information, life cycle assessment data and evidences.
Valid to
The EPD was created according to the specifications of EN 15804+A2. In
25.06.2028 the following, the standard will be simplified as EN 15804.
Verification
The standard EN 15804 serves as the core PCR
Independent verification of the declaration and data according to ISO
14025:2011
internally X externally
Dipl.-Ing. Hans Peters
(Chairman of Institut Bauen und Umwelt e.V.)
Dipl.-Ing. Hans Peters Dr Naeem Adibi,
(Managing Director Institut Bauen und Umwelt e.V.) (Independent verifier)
1 Environmental Product Declaration - Knauf Integral KG - Knauf GIFAfloor DB 40 green
Product
Product description/Product definition This product contains other CMR substances in categories 1A
The declared product Knauf GIFAfloor DB 40 green is a or 1B (Regulation (EC) No. 1272/2008) which are not on the
gypsum fibre board made of gypsum with paper fibres candidate list, exceeding 0.1 percentage by mass: no
suspended in the gypsum matrix for reinforcement of the
boards. The declared products have a thickness of 40 mm. Biocide products were added to this construction product or it
Further thicknesses (30 mm, 36 mm) are declared in separate has been treated with biocide products (this then concerns a
EPDs. treated product as defined by the (EU) Ordinance on Biocide
Products No. 528/2012): no
For the placing on the market of the product in the European
Union/European Free Trade Association (EU/EFTA) (with the Reference service life
exception of Switzerland) Regulation (EU) No. 305/2011 (CPR) No reference service life according to ISO 15686 has been
applies. The product needs a declaration of performance determined for the declared products. However, a service life of
taking into consideration EN 15283-2:2008 + A1:2009, Gypsum ≥ 50 years can be assumed for raised access floor panels
boards with fibrous reinforcement - Definitions, according to the BBSR table "Service lives of components for
requirements and test methods - Part 2: Gypsum fibre boards life cycle assessment according to BNB" (code no. 352.911).
and the CE-marking. There are no influences on ageing when the panels are applied
in accordance with the rules of technology.
National provisions apply for the application and use.
Extraordinary effects
Application
Knauf GIFAfloor DB green boards are used as raised access
floors panels with loose laid carpets or for access openings in Fire protection
dry hollow floor systems. Building material class A1
Applicable standards are: Burning droplets -
• EN 12825:2001, Raised access floors Smoke gas development -
• EN 13213:2001, Hollow floors
Contact with water
Technical Data Knauf GIFAfloor DB 30 green are designed to tolerate relative
Technical datasheets can be downloaded from the website humidities up to 75 %. Exceeding humidities or permanent
https://www.knauf-integral.de. exposure to wet conditions may lead to a decrease in strength
and should be avoided. However, due to the ingredients no
Constructional data of Knauf GIFAfloor DB 40 green
negative effect on human health is to be expected from
Name Value Unit
leaching.
Gross density acc. to EN 15283-2 ≥ 1500 kg/m3
Thermal conductivity acc. to EN ISO 10456 0.25 W/mK An instruction sheet about the restoration of flood damage is
available under www.knauf.de /BSDH/. Information about the
Calculation value for thermal conductivity 0.44 W/mK
removal of flood damage can also be downloaded from
Specific heat capacity 1 kJ/kgK
www.gypsum.org.
Water vapour diffusion resistance factor acc. to 10 - Due to the loose laying of Knauf GIFAfloor DB green panels
EN ISO 10546 affected panels can be easily replaced by new ones.
Water vapour diffusion resistance factor acc. to
4 -
EN ISO 10546 Re-use phase
0.5 - Knauf GIFAfloor DB 40 green panels are laid loosely on the
Moisture content at 20 °C, 65% humidity M.-%
0.9 sub-construction and is typically covered by self-laid loose
textile covering. Therefore, they can be removed without any
Elongation/Vibration when humidity changes by
≤ 1.00 mm/m damage to the panels and re-use is possible.
30% (20°C) acc. to EN 318
Performance data of the product in accordance with the According to the German Commercial Waste Ordinance
declaration of performance with respect to its essential GewAbfV construction and demolition based on gypsum is
characteristics according to EN 15283-2:2008 + A1:2009, preferably collected separately from other waste types and
Gypsum boards with fibrous reinforcement - Definitions, supplied to recycling facilities. In addition, Knauf GIFAfloor DB
requirements, and test methods - Part 2: Gypsum fibre boards. 40 green panels are designed to be easily recyclable.
Base materials/Ancillary materials
Disposal
Knauf GIFAfloor DB green panels consist of approx. 92 % w/w
Knauf GIFAfloor DB 40 green panels need to be dismanteled
set gypsum reinforced with > 7 % w/w paper fibres and < 0.5 %
and collected separately from other construction waste. If
additives. Knauf GIFAfloor DB green panels are impregnated
disposed, Knauf GIFAfloor DB 40 green panels need to be
with < 0.5 % w/w impregnating agent (surface
disposed of as gypsum waste under the European Waste Code
impregnation).
(EWC)
The declared products contains substances listed in the
17 08 02 - gypsum-based construction materials other than
candidate list (date: 17.01.2023, ECHA) exceeding 0.1
those mentioned in 17 08 01
percentage by mass: no.
LCA: Calculation rules
2 Environmental Product Declaration - Knauf Integral KG - Knauf GIFAfloor DB 40 green
crystallization into the crystal lattice of calcium sulphate. That
Declared Unit way, gypsum becomes settled and hardened. Redundant
The declared unit is 1 m² of Knauf GIFAfloor DB 40 green surface water is finally removed in a dryer.
panels. The conversion factors and densities are given in the
table below:
Declared unit for Knauf GIFAfloor DB 40 green Cut-offs
Name Value Unit
Cut-off rules as required by EN 15804+A2 are respected. The
Declared unit 1 m2 details are given in the background report. The environmental
conversion factor [Mass/Declared Unit] to 1 kg 0.016 - impacts imposed by these cut-offs are considered neglectable.
Gross density - kg/m3 In total, the cut off materials and processes are less than 5 % of
the mass and energy flows in the modules (A1-A3).
Grammage 64.4 kg/m2
Layer thickness 0.04 m Data quality
The declared environmental impacts are average impacts for Datasets exclusively from GaBi databases (version 2022.1) are
the production in plant Satteldorf. Water and energy used for the LCA modelling. All datasets used have been
consumption is measured on an annual basis and allocated to updated in the last 5 years. For processes and materials, where
the various products by the annually produced surface area per no direct match is available, data from literature or expert
panel thickness. judgements are applied. Only a few materials and processes
needed to be cut off due to missing information. Since these
Knauf Integral plant Satteldorf is specifically designed to cut-off materials and processes are only of small amounts (<< 1
produce a fibre reinforced gypsum material called Knauf % w/w), the total influence of these neglected inputs is
GIFAtec which is adapted in shape, density, surface treatment, expected to be lower than 5 % of energy usage and mass.
and edge trimming to yield the desired products. Therefore,
results of the life cycle indicators are considered to be very With respect to technological, geographic and time
robust. representativeness, the overall data quality is evaluated to be
'satisfactory'.
The LCA was modeled with software GaBi and its
corresponding databases (database version 2022.1). Foreground data are related to production data from plant
Satteldorf for the reference year 2020. Water and energy
System boundary consumption are monitored and reported on an annual basis
Type of the EPD: cradle to gate - with options, modules C1–C4, and allocated to the specific products based on annually
and module D (A1–A3 + C+ D, additional modules: A4, A5) produced surface area per panel thickness. Since the
composition of the material is quite constant throughout the
This EPD includes the following life cycle stages: product range, the LCA results are considered to be quite
robust with respect to the foreground data.
• provision of raw materials and transport to plant
Satteldorf, production of boards (A1-A3) including
Allocations
thermal energy for calcination and drying (from natural
Allocations in the foreground data have only been applied for
gas, geographic scope: DE), as well as electricity
energy and water consumption data which is monitored on an
(residual mix DE)
annual basis for the whole production plant Satteldorf.
• transport to building site (A4)
Allocations in the background data are described and have not
• installation at building site (A5) including the incineration
been adjusted. Paper fibres incorporated in the gypsum fibre
of transport packaging
panels are made from waste cardboard and enter the product
• manual disassembly (C1)
system free of burdens.
• transport to recycling facility or landfill site (C2)
• 2 scenarios for end of life:
Further allocations of production data have been avoided.
• Scenario 1: landfilling (C4/1), corresponding to zero
However, there may be allocations in the background data
impacts in C3/1 and credits in D/1 from incineration of
which are are explained in the documentation of the respective
packaging material in A5
datasets.
• Scenario 2: recycling (C3/2), zero impacts in C4/2 and
credits for the recycled material beyond the system
Geographic Representativeness
boundaries and from A5 (D/2). Recycling includes the
Land or region, in which the declared product system is
electrical energy for the crushing and grinding of the
manufactured, used or handled at the end of the product´s
disassembled panels prior to backfeeding into the next
lifespan: Global
production cycle.
Fig. 1 illustrates the production process: Natural and Flue gas Comparability
desulphurization (FGD) gypsum is calcined (removal of water of Basically, a comparison or an evaluation of EPD data is only
crystallization). The calcined stucco in mixed with additive and possible if all the data sets to be compared were created
fibres from wastepaper and mixed with water. This slurry is fed according to EN 15804 and the building context, respectively
to an infinite belt with vacuum pumps. After this, the density of the product-specific characteristics of performance, are taken
the material is adjusted by a winding roller and a press. Mixing into account.
with water leads to the re-incorporation of water of
3 Environmental Product Declaration - Knauf Integral KG - Knauf GIFAfloor DB 40 green
4 Environmental Product Declaration - Knauf Integral KG - Knauf GIFAfloor DB 40 green
Fig. 1: Production process for gypsum fibre panels
LCA: Scenarios and additional technical information
transport of the declared products by inter-/extrapolating
Characteristic product properties of biogenic carbon distances and mixing of transport means according to
Information on describing the biogenic Carbon Content at the conditions at hand for individual building assessments.
factory gate
However, since Knauf GIFAfloor DB green panels are shipped
Name ValueUnit
globally, further transportation scenarios were considered:
kg
Biogenic carbon content in product 2.52 - Scenario (A4/1): Transport by truck 1000 km
C
- Scenario (A4/2): Transport by rail 1000 km
Biogenic carbon content in accompanying kg - Scenario (A4/3): Transport by ocean freight ship over 10000
0.102
packaging C km
- Scenario (A4/4): Transport by river freight ship over 1000 km
The results of these further transportation scenarios are given
Product Stage (A1-A3)
in the Annexe to this EPD.
Supply of raw materials
Default scenario (A4): Transport by truck 500 km
Knauf GIFAfloor DB green boards are gypsum fibre boards
consisting of gypsum with cellulose fibre from recycled Name Value Unit
cardboard incorporated in the gypsum matrix. Currently, natural Litres of fuel 0.113 l/100km
gypsum from open-cast mining in close vicinity to the
Transport distance 500 km
production plant as well as gypsum from the flue gas
Capacity utilisation (including empty runs) 50 %
desulphurization of different coal fired power plants is used to
produce the boards. Gross density of products transported ≥ 1500 kg/m3
Installation into the building (A5)
Small amounts of additives are used for easier processing and
fine adjustment of properties. Raised access floor panels Knauf GIFAfloor DB green are
installed by being loosely laid on specific raised access floor
pedestals available at Knauf Integral KG according to
Transport of raw materials the installation instructions. No sealing of joints is required.
Natural gypsum is extracted from mines close to the Name Value Unit
manufacturing sites. Accordingly, transport distances are short Electricity consumption - kWh
(< 30 km) and trucks are used. FGD gypsum is transported by
Type of assembly manually
truck from coal-fired power plants in Germany and Europe,
Construction waste 5 %
mainly. In few cases, a river freight ship and even an ocean
freight ship are required for transportation. Due to these Treatment of packaging
incineration
different transportation vehicles employed, the transport waste
distances for FGD gypsum were calculated with weighted Components not Substructures, screws, jointing
averages for a combined transportation by truck, river, and considered material
ocean.
Use phase (B1-B7): Excluded since no environmental
Further raw materials are supplied by truck from manufacturers
impacts/benefits are expected.
within Germany or from neighbouring countries.
A service life of ≥ 50 years can be assumed for raised access
Manufacturing
floor panels and ceiling and wall coverings according to the
Gypsum (natural and FGD gypsum) is calcined to stucco before
BBSR table "Service lives of components for life cycle
mixing with water. Stucco, cellulose fibres and small amounts of
assessment according to BNB".
additives are then suspended in water to give a slurry. The
resulting mixture passes a job feeder and is fed on an infinite
Hygrothermal in-use conditions (stationary): -10 °C to +35 °C;
felt with vacuum pumps to remove excess water. Afterwards,
35 to 75 % rel. air humidity
the pulp is driven through a winding roller and a subsequent
press for panel forming and further removal of water before it End of life (C1-C4)
finally enters a dryer. Drying of surface moisture is followed by Knauf GIFAfloor DB 40 green are disassembled manually and
surface finishing, formatting and edge processing as well as the collected separately from other deconstruction waste.
application of the impregnating agent. Transportation in C2 is assumed to be 100 km by truck to either
an appropriate landfill site (scenario 1) or to a recycling facility
(Transport) Packaging (scenario 2).
Knauf GIFAfloor DB green panels are not packaged individually, Since Knauf GIFAfloor DB 40 green are laid loosely, no
but stacked on a wooden pallet (reusable), covered with a adhering foreign material needs to be removed from the panels
cardboard sheet and secured with PET straps. prior to recycling (scenario 2). The panels are milled to fine
powder without any further material separation. The same
energy consumption as for the milling of natural gypsum in
Transport to the building site (A4)
plant Satteldorf is assumed for the recycling procedure. The
As the default value, transportation over 500 km by truck was
recycled gypsum is assumed to replace virgin FGD and natural
assumed for the transportation of the products to the building
gypsum in the same ratio as it was initially introduced into
site. This is no actual transport distance since transport
production cycle declared in modules A1-A3.
distances can only be considered at the building level.
Nevertheless, the provided numbers shall enable the
calculation of the actual environmental burdens for the
5 Environmental Product Declaration - Knauf Integral KG - Knauf GIFAfloor DB 40 green
Name ValueUnit of packaging material (results only from A5)
D/2: contains credits for exported energy from incineration of
Collected separately gypsum-based construction
64.4 kg packaging material in A5 and the benefits from the recycled
materials
material of Knauf GIFAfloor DB green panels replacing FGD
Landfilling scenario 1 64.4 kg
and natural gypsum in the same ratio as both gypsum types
Recycling scenario 2 64.4 kg
were introduced in A1-A3; amount of paper fibres is discounted
With the definition of 2 end-of-life scenarios, benefits and loads from weight of demolition waste to avoid double counting of
beyond system boundaries are declared as follows: secondary material and replacement of gypsum by paper fibres
D/1: contains only credits for exported energy from incineration
6 Environmental Product Declaration - Knauf Integral KG - Knauf GIFAfloor DB 40 green
LCA: Results
Note: Two scenarios for the end of life stage were considered as 100 % scenario, each.
Scenario 1: Landfilling - module C4/1, C3/1 with zero impacts, D/1 (only from A5)
Scenario 2: Recycling - module C3/2, C4/2 with zero impacts, D/2 (from A5 and C3/2)
DESCRIPTION OF THE SYSTEM BOUNDARY (X = INCLUDED IN LCA; ND = MODULE OR INDICATOR NOT DECLARED; MNR =
MODULE NOT RELEVANT)
Benefits and
Construction loads beyond
Product stage Use stage End-of-life stage
process stage the system
boundaries
la ire ta m w a Ry lp p u s tro p s n a rT g n iru tc a fu n a M e h t m o rf tro p s n a rTe tis e h t o t e ta g y lb m e s s A e s U e c n a n e tn ia M ria p e R tn e m e c a lp e R tn e m h s ib ru fe R y g re n e la n o ita re p Oe s u re ta w la n o ita re p Oe s u n o itc u rts n o c -e Dn o itilo m e d tro p s n a rT g n is s e c o rp e ts a W la s o p s iD -e s u e R-y re v o c e R-g n ilc y c e Rla itn e to p
A1 A2 A3 A4 A5 B1 B2 B3 B4 B5 B6 B7 C1 C2 C3 C4 D
X X X X X MND MND MNR MNR MNR MND MND X X X X X
RESULTS OF THE LCA - ENVIRONMENTAL IMPACT according to EN 15804+A2: 1 m² Knauf GIFAfloor DB 40 green, 64.4 kg/m²,
40 mm
Parameter Unit A1-A3 A4 A5 C1 C2 C3/1 C3/2 C4/1 C4/2 D/1 D/2
GWP-total kg CO 2 eq 8.63E-01 2.27E+00 1.48E+00 0 4.58E-01 0 9.29E+00 1.05E+01 0 -1.35E-01 -9.57E+00
GWP-fossil kg CO 2 eq 1.04E+01 2.26E+00 7.39E-01 0 4.55E-01 0 6.63E-02 1.25E+00 0 -1.35E-01 -3.37E-01
GWP-
biogenic kg CO 2 eq -9.59E+00 0 7.45E-01 0 0 0 9.23E+00 9.22E+00 0 -6.89E-04 -9.23E+00
GWP-luluc kg CO 2 eq 2.11E-03 8.62E-03 7.8E-04 0 3.05E-03 0 1.4E-05 1.81E-03 0 -1.48E-05 -1.83E-04
kg CFC11
ODP 2.39E-11 5.16E-13 1.38E-12 0 5.59E-14 0 9.7E-13 2.57E-12 0 -9.1E-13 -1.55E-12
eq
AP mol H+ eq 3.53E-02 2.19E-03 2.36E-03 0 5.12E-04 0 1.45E-04 8.04E-03 0 -1.77E-04 -6.83E-04
EP-
kg P eq 3.3E-06 4.49E-06 2.51E-06 0 1.62E-06 0 1.93E-07 4.06E-05 0 -1.85E-07 -4.05E-07
freshwater
EP-marine kg N eq 1.02E-02 7.66E-04 7.12E-04 0 1.71E-04 0 3.26E-05 2.64E-03 0 -4.8E-05 -2.48E-04
EP-terrestrial mol N eq 1.14E-01 8.75E-03 7.73E-03 0 1.98E-03 0 3.42E-04 2.39E-02 0 -5.15E-04 -2.81E-03
kg NMVOC
POCP 2.84E-02 1.96E-03 2.03E-03 0 4.42E-04 0 8.82E-05 8.6E-03 0 -1.34E-04 -6.61E-04
eq
ADPE kg Sb eq 2.67E-06 2.27E-07 1.54E-07 0 4.61E-08 0 1.81E-08 1.16E-07 0 -2.03E-08 -3.88E-08
ADPF MJ 1.49E+02 2.99E+01 1.02E+01 0 6E+00 0 1.2E+00 1.66E+01 0 -2.29E+00 -4.54E+00
m3 world eq
WDP 6.25E-01 1.07E-02 8.17E-02 0 5.28E-03 0 1.51E-02 1.22E-01 0 -1.43E-02 -1.66E-02
deprived
GWP = Global warming potential; ODP = Depletion potential of the stratospheric ozone layer; AP = Acidification potential of land and water; EP =
Eutrophication potential; POCP = Formation potential of tropospheric ozone photochemical oxidants; ADPE = Abiotic depletion potential for non-fossil
resources; ADPF = Abiotic depletion potential for fossil resources; WDP = Water (user) deprivation potential)
RESULTS OF THE LCA - INDICATORS TO DESCRIBE RESOURCE USE according to EN 15804+A2: 1 m² Knauf GIFAfloor DB
40 green, 64.4 kg/m², 40 mm
Parameter Unit A1-A3 A4 A5 C1 C2 C3/1 C3/2 C4/1 C4/2 D/1 D/2
PERE MJ 4.62E+00 1.98E+00 8.51E+00 0 4.17E-01 0 8.52E+01 2.16E+00 0 -6.29E-01 -8.55E+01
PERM MJ 8.81E+01 0 -3.63E+00 0 0 0 -8.45E+01 0 0 0 8.45E+01
PERT MJ 9.28E+01 1.98E+00 4.89E+00 0 4.17E-01 0 6.68E-01 2.16E+00 0 -6.29E-01 -9.57E-01
PENRE MJ 1.49E+02 3E+01 1.03E+01 0 6.03E+00 0 1.2E+00 1.66E+01 0 -2.29E+00 -4.54E+00
PENRM MJ 1.11E-01 0 -1.11E-01 0 0 0 0 0 0 0 ND
PENRT MJ 1.49E+02 3E+01 1.02E+01 0 6.03E+00 0 1.2E+00 1.66E+01 0 -2.29E+00 -4.54E+00
SM kg 4.9E+00 0 0 0 0 0 0 0 0 0 -5.94E+01
RSF MJ 0 0 0 0 0 0 0 0 0 0 0
NRSF MJ 0 0 0 0 0 0 0 0 0 0 0
FW m3 2.72E-02 1.57E-03 2.67E-03 0 4.88E-04 0 6.37E-04 3.68E-03 0 -6.05E-04 -9.96E-04
PERE = Use of renewable primary energy excluding renewable primary energy resources used as raw materials; PERM = Use of renewable primary
energy resources used as raw materials; PERT = Total use of renewable primary energy resources; PENRE = Use of non-renewable primary energy
excluding non-renewable primary energy resources used as raw materials; PENRM = Use of non-renewable primary energy resources used as raw
materials; PENRT = Total use of non-renewable primary energy resources; SM = Use of secondary material; RSF = Use of renewable secondary fuels;
NRSF = Use of non-renewable secondary fuels; FW = Use of net fresh water
RESULTS OF THE LCA – WASTE CATEGORIES AND OUTPUT FLOWS according to EN 15804+A2:
1 m² Knauf GIFAfloor DB 40 green, 64.4 kg/m², 40 mm
Parameter Unit A1-A3 A4 A5 C1 C2 C3/1 C3/2 C4/1 C4/2 D/1 D/2
HWD kg 2.65E-08 1.91E-10 1.41E-09 0 4.39E-11 0 1.04E-10 1.36E-09 0 -3.1E-10 -3.62E-10
NHWD kg 8.54E-02 4.94E-03 3.16E+00 0 9.94E-04 0 9.06E-04 6.31E+01 0 -1.16E-03 -2.05E-03
7 Environmental Product Declaration - Knauf Integral KG - Knauf GIFAfloor DB 40 green
RWD kg 6.07E-03 4.03E-05 3.21E-04 0 1.17E-05 0 1.92E-04 1.88E-04 0 -1.8E-04 -2.15E-04
CRU kg 0 0 0 0 0 0 0 0 0 0 0
MFR kg 0 0 0 0 0 0 6.43E+01 0 0 0 0
MER kg 0 0 0 0 0 0 0 0 0 0 0
EEE MJ 0 0 6.05E-01 0 0 0 0 0 0 0 0
EET MJ 0 0 1.09E+00 0 0 0 0 0 0 0 0
HWD = Hazardous waste disposed; NHWD = Non-hazardous waste disposed; RWD = Radioactive waste disposed; CRU = Components for re-use;
MFR = Materials for recycling; MER = Materials for energy recovery; EEE = Exported electrical energy; EET = Exported thermal energy
RESULTS OF THE LCA – additional impact categories according to EN 15804+A2-optional:
1 m² Knauf GIFAfloor DB 40 green, 64.4 kg/m², 40 mm
Parameter Unit A1-A3 A4 A5 C1 C2 C3/1 C3/2 C4/1 C4/2 D/1 D/2
Disease
PM 1.06E-06 1.39E-08 5.87E-08 0 3.51E-09 0 1.21E-09 9.41E-08 0 -1.47E-09 -4.63E-07
incidence
IR kBq U235 eq 4.79E-01 4.1E-03 2.62E-02 0 1.73E-03 0 3.26E-02 2.28E-02 0 -3.05E-02 -3.41E-02
ETP-fw CTUe 5.7E+01 2.28E+01 4.8E+00 0 4.23E+00 0 5.27E-01 1.12E+01 0 -5.03E-01 -1.32E+00
HTP-c CTUh 1.61E-09 4.57E-10 1.71E-10 0 8.72E-11 0 1.51E-11 1.2E-09 0 -2.31E-11 -4.29E-11
HTP-nc CTUh 1.32E-07 2.3E-08 1.49E-08 0 4.73E-09 0 5.53E-10 1.36E-07 0 -8.87E-10 -2.1E-09
SQP SQP 6.07E+01 8.91E+00 3.78E+00 0 2.52E+00 0 4.34E-01 2.88E+00 0 -4.08E-01 -1.12E+00
PM = Potential incidence of disease due to PM emissions; IR = Potential Human exposure efficiency relative to U235; ETP-fw = Potential comparative
Toxic Unit for ecosystems; HTP-c = Potential comparative Toxic Unit for humans (cancerogenic); HTP-nc = Potential comparative Toxic Unit for humans
(not cancerogenic); SQP = Potential soil quality index
Disclaimer 1 – for the indicator “Potential Human exposure efficiency relative to U235”. This impact category deals mainly with the
eventual impact of low dose ionizing radiation on human health of the nuclear fuel cycle. It does not consider effects due to possible
nuclear accidents, occupational exposure nor due to radioactive waste disposal in underground facilities. Potential ionizing radiation
from the soil, from radon and from some construction materials is also not measured by this indicator.
Disclaimer 2 – for the indicators “abiotic depletion potential for non-fossil resources”, “abiotic depletion potential for fossil resources”,
“water (user) deprivation potential, deprivation-weighted water consumption”, “potential comparative toxic unit for ecosystems”,
“potential comparative toxic unit for humans – cancerogenic”, “Potential comparative toxic unit for humans - not cancerogenic”,
“potential soil quality index”. The results of this environmental impact indicator shall be used with care as the uncertainties on these
results are high or as there is limited experienced with the indicator.
References
Standards ISO 14025
DIN EN ISO 14025:2011-10, Environmental labels
EN 318 and declarations — Type III environmental declarations
EN 318:2002-06 Wood-based panels - Determination of — Principles and procedures.
dimensional changes associated with changes in relative
humidity ISO 14040
ISO 14040:2006 + Amd 1:2020, Environmental management –
EN ISO 10456 Life cycle assessment – Principles and framework
EN ISO 10456:2010-05, Building materials and products -
Hygrothermal properties - Tabulated design values
and procedures for determining declared and design thermal ISO 14044
values (ISO 10456:2007 + Cor. 1:2009) ISO 14044:2006 + Amd 1:2017 + Amd 2:2020,
Environmental management – Life cycle assessment –
EN 12825 Requirements and guidelines
EN 12825:2001, Raised access floors
ISO 15686
EN 13213 ISO 15686-2:2012-05, Buildings and constructed assets -
EN 13213:2001, Hollow floors Service life planning - Part 2: Service life prediction procedures
EN 13501 Further References
EN 13501-1: 2018, Fire classification of construction
products and building elements - Part 1: Classification using BBSR
data from reaction to fire tests table "Service lives of components for life cycle
assessment according to BNB"
EN 15283 http://www.nachhaltigesbauen.de/baustoffund-
EN 15283-2:2008 + A1:2009, Gypsum boards with gebaeudedaten/nutzungsdauern-von-bauteilen.html, published
fibrous reinforcement - Definitions, requirements, and test 2017, last accessed 2022-09-29
methods -
Part 2: Gypsum fibre boards ECHA
European Chemicals Agency (ECHA), Candidate List
EN 15804 of Substances of Very High Concern for Authorisation
EN 15804:2019+A2, Sustainability of construction works (published in
— Environmental Product Declarations — Core rules for the accordance with Article 59(10) of the REACH
product category of construction products. Regulation), http://echa.europa.eu/de/candidate-list-table,
Revision: 2023-
8 Environmental Product Declaration - Knauf Integral KG - Knauf GIFAfloor DB 40 green
01-17 Rules for the Life Cycle Assessment and Requirements on
the Project Report according to EN 15804+A2:2019, v1.1.2,
European Waste Code 2021-09-02
Guidance on classification of waste according to EWC-
Stat categories, Supplement to the Manual for the IBU PCR Part B "Plasterboards"
Implementation of the Regulation (EC) No 2150/2002 on Institut Bauen und Umwelt e.V.: PCR Guidance-Texts
Waste Statistics, COMMISSION OF THE for Building-Related Products and Services Part B:
EUROPEAN COMMUNITIES/EUROSTAT, v2, December 2010 Requirements on the EPD for Plasterboard, v1.7, 2019-01-04
GaBi (EU) Ordinance on Biocide Products No. 528/2012
GaBi ts (v10.6.1.35): Software-System and Databases for REGULATION (EU) No 528/2012 OF THE
Life Cycle Engineering, Sphera Solutions GmbH, Leinfelden- EUROPEAN PARLIAMENT AND OF THE COUNCIL of 22 May
Echterdingen, Germany, 2022 (database version 2022.1) 2012 concerning the making available on the market and use
of biocidal products
GewAbfV
Verordnung über die Bewirtschaftung von
gewerblichen Siedlungsabfällen und von bestimmten Bau- Regulation (EU) No. 305/2011
und Abbruchabfällen (Gewerbeabfallverordnung - GewAbfV) REGULATION (EU) No 305/2011 OF THE
Gewerbeabfallverordnung vom 18. April 2017 (BGBl. I S. 896), EUROPEAN PARLIAMENT AND OF THE COUNCIL of 9 March
last amended by Artikel 3 der Verordnung vom 28. April 2022 2011 laying down harmonised conditions for the marketing
(BGBl. I S. 700) of construction products and repealing Council
German Commercial Waste Ordinance Directive 89/106/EEC
IBU 2021 Regulation (EC) No. 1272/2008
Institut Bauen und Umwelt e.V.: Allgemeine Anleitung für REGULATION (EC) No 1272/2008 OF THE
das EPD-Programm des Institut Bauen und Umwelt e.V. (IBU). EUROPEAN PARLIAMENT AND OF THE COUNCIL of 16
Version 2.0, Berlin: Institut Bauen und Umwelt e.V., 2021. December 2008 on classification, labelling and packaging of
www.ibu-epd.com substances and mixtures, amending and repealing Directives
67/548/EEC and 1999/45/EC, and amending Regulation (EC)
IBU PCR Part A No 1907/2006
Institut Bauen und Umwelt e.V.: Product Category Rules
for Building-Related Products and Services Part A: Calculation
9 Environmental Product Declaration - Knauf Integral KG - Knauf GIFAfloor DB 40 green
Publisher
Institut Bauen und Umwelt e.V. +49 (0)30 3087748- 0
Hegelplatz 1 info@ibu-epd.com
10117 Berlin www.ibu-epd.com
Germany
Programme holder
Institut Bauen und Umwelt e.V. +49 (0)30 3087748- 0
Hegelplatz 1 info@ibu-epd.com
10117 Berlin www.ibu-epd.com
Germany
Author of the Life Cycle Assessment
Knauf Gips KG 0049 9001 31-1000 *
Am Bahnhof 7 knauf-direkt@knauf.de
97346 Iphofen www.knauf.de
Germany
Owner of the Declaration
Knauf Integral KG +49 (7951) 497-0
Am Bahnhof 16 info@knauf-integral.de
74589 Satteldorf https://www.knauf-integral.de/de/
Germany
10 Environmental Product Declaration - Knauf Integral KG - Knauf GIFAfloor DB 40 green
