ENVIRONMENTAL PRODUCT DECLARATION
as per ISO 14025 and EN 15804+A2
Owner of the Declaration VELUX Group
Publisher Institut Bauen und Umwelt e.V. (IBU)
Programme holder Institut Bauen und Umwelt e.V. (IBU)
Declaration number EPD-VEL-20240210-IBA1-EN
Issue date 23.07.2024
Valid to 22.07.2029
VELUX Commercial acrylic dome rooflights (Akrylovenlys)
VELUX Group
www.ibu-epd.com | https://epd-online.com
1. General Information
VELUX Group VELUX Commercial acrylic dome rooflights
(Akrylovenlys)
Programme holder Owner of the declaration
IBU – Institut Bauen und Umwelt e.V. VELUX Group
Hegelplatz 1 Ådalsvej 99
10117 Berlin 2970 Hørsholm
Germany Denmark
Declaration number Declared product / declared unit
EPD­VEL­20240210­IBA1­EN 1 m2 of VELUX Commercial acrylic dome rooflights (Akrylovenlys).
This declaration is based on the product category rules: Scope:
Windows and doors , 01.08.2021 The LCA represents 100% of the production volume of VELUX
(PCR checked and approved by the SVR) Commercial acrylic dome rooflights produced by VELUX Commerical in
Kongerslev (DK).
The owner of the declaration shall be liable for the underlying information
Issue date and evidence; the IBU shall not be liable with respect to manufacturer
information, life cycle assessment data and evidences.
23.07.2024
The EPD was created according to the specifications of EN 15804+A2. In
the following, the standard will be simplified as EN 15804.
Valid to
22.07.2029 Verification
The standard EN 15804 serves as the core PCR
Independent verification of the declaration and data according to ISO
14025:2011
internally X externally
Dipl.­Ing. Hans Peters
(Chairman of Institut Bauen und Umwelt e.V.)
Florian Pronold Dr.­Ing. Nikolay Minkov,
(Managing Director Institut Bauen und Umwelt e.V.) (Independent verifier)
1 Environmental Product Declaration ­ VELUX Group ­ VELUX Commercial acrylic dome rooflights (Akrylovenlys)
2. Product
Name Value Unit
2.1 Product description/Product definition
Resistance to upward load NPD
The declared acrylic domes are 2­3­4­5 layer plastic rooflights
Resistance to downward load NPD
in either dome or pyramid shape. The outer layer is made in
acrylic (PMMA) or polycarbonate material (PC) with inner layers Reaction to fire, upstand acc. EN 13501 D­s2, d0
of acrylic (PMMA). The dome is framed by aluminum profile in Reaction to fire, top: PMMA acc. EN 13501 E
either black, grey or white. Reaction to fire, top: PC acc. EN 13501 B­s1, d0
The upstand is made of either insulated plywood put together in
Reaction ot fire, top: PMMA+PC acc. EN
a sandwich construction or as massive rafter wood. E
13501
For the placing on the market of the product in the European
Resistance to fire NPD
Union/European Free Trade Association (EU/EFTA) (with the
exception of Switzerland) Regulation (EU) No. 305/2011 (CPR) External fire performance NPD
applies. The product needs a declaration of performance taking Water tightness NPD
into consideration: Small, hard body NPD
• EN 1873:2005, Prefabricated accessories for roofing - Large, soft body acc. EN 1873 SB 1200
Individual rooflights of plastics - Product specification Direct airborne sound insulation 20 ­ 22 dB
and test methods
W/(m²
and the CE­marking. Thermal transmittance acc. EN 1873 1.2­2.0
K)
2.2 Application Luminous transmittance; clear layer(s) acc. 68 % ­ 82
VELUX Commercial acrylic domes are intended for the lighting EN 1873 %
by means of daylight and of ventilating interior spaces by Luminous transmittance; opal layer added 64 % ­ 77
means of opening devices acc. EN 1873 %
Areas of application for the VELUX Commercial acrylic domes Air permieability NPD
are: Durability NPD
• heated industrial buildings
NPD: no performance declared
• warehouses
Thermal transmittance calculated for insulated upstand 30 cm
• small production factory
above roof construction, for size 120 cm x 120 c, based on
• car service/mechanics
worst case openable units with curved dome
• stock facility
• sport facilities incl. locker rooms
Performance data of the product in accordance with the
• temporary houses
declaration of performance with respect to its essential
exhibition area
characteristics according to:
• wholesale
• EN 1873:2005, Prefabricated accessories for roofing -
• schools & day cares
Individual rooflights of plastics - Product specification
• railway stations
and test methods.
2.3 Technical Data
2.4 Delivery status
Technical characteristics
VELUX Commercial domes are avilable in sizes ranging from
Technical characteristics listed according to DoP No. 457503-2 520 mm x 520 mm (0.27 m2) to 1200 mm x 2400 mm (2.9 m2)
for Acrylic/Polycarbonate rooflight, Curved or Pyramid dome with a standard size of 850 mm x 850 mm (0.72 m2). The height
Types 20­H­­, 30­H­­, 40­H­­, 50­H­­, 20­P­­, 30­P, 40­P­­, 50­P
can range from 100 mm to 1000 mm with a standard height of
— with insulating upstand type I48:
300 mm.
2.5 Base materials/Ancillary materials
The delcared product is composed of:
Name Value Unit
Poly(methyl methacylate) (PMMA) 32 % ­
Polycarbonate (PC) 30 % ­
Plywood 18 % ­
Sawn timber 12 % ­
Stone wool 3 %
Aluminium 2 %
Steel 2 %
Others 1 % ­
1. This product/article/at least one partial article contains
substances listed in the ECHA candidate list (date: 15.08.2023)
exceeding 0.1 percentage by mass: no.
2. This product/article/at least one partial article contains other
carcinogenic, mutagenic or reprotoxic (CMR) substances in
categories 1A or 1B which are not on the ECHA candidate list,
2 Environmental Product Declaration ­ VELUX Group ­ VELUX Commercial acrylic dome rooflights (Akrylovenlys)
exceeding 0.1 percentage by mass: not investigated with
suppliers. 2.11 Environment and health during use
VELUX Commercial acrylic domes do not contain any
3. Biocide products were added to this construction product or it pollutants that could be released during use.
has been treated with biocide products (this then concerns a
treated product as defined by the (EU) Ordinance on Biocide Environmental protection: According to current knowledge,
Products No. 528/2012): no. hazards to water, air and soil cannot arise when the products
are used as intended.
2.6 Manufacture
All the raw materials including wood, plywood, polycarbonate, Health protection: According to current knowledge, no health
acrylic, aluminium, actuators and all ancillary materials (fittings, hazards or impairments are to be expected.
screws, glue, plastic parts, gasket, etc.) are bought from
external suppliers. First the wood and plywood are cross­cut for 2.12 Reference service life
the production of the upstands; in addition, all aluminium parts It is not possible to calculate the reference service life
are cross­cut, drilled and welded; in a last preparatory step, the according to ISO 15686. The service life based on a
polycarbonate and the acrylic are crosscut and shaped. All the manufacturer's declaration is 30 years. The corresponding
components are then assembled to the final product, which utilization scenario is declared in chapter 4.
undergoes a final inspection.
2.13 Extraordinary effects
Only a few items are bought manufactured from a sub supplier.
That is the aluminium sheets for windscreens and standard Fire
sizes frames for insulated upstands. Also the wood for solid See table 2.3 for the reaction to fire of the different
frames (Kehlet) is bought from external. components.
Normally aluminium is not surface treated; sometimes the
aluminium parts are painted (wet paint) from a local dealer, but Water
not very often. In the event of unforeseen exposure to water (flood), no
The insulated upstand made from wood/plywood come usually adverse effects on human health or the environment are to be
as laminated material; only in a few cases, the interior side of expected.
the upstands are painted.
In order to guarantee the quality assurance of the product, Mechanical destruction
VELUX operates a quality management system according to In the event of unforeseen mechanical destruction, VELUX
ISO 9001. Commercial acrylic domes must be replaced; no adverse
effects on human health or the environment are to be expected.
2.7 Environment and health during manufacturing
2.14 Re-use phase
The health of employees is protected by suitable measures
specified by the authorities. These include safety goggles, VELUX Commercial acrylic domes can be dismantled manually
hearing protection, helmets, gloves, safety shoes, etc. without any problems. The metal parts are usually recycled,
Waste generated during every process in the company is and the wooden and plastic parts are sent for thermal recycling
collected, sorted and disposed of in a professional and for energy recovery.
resource­conserving manner.
2.15 Disposal
2.8 Product processing/Installation VELUX Commercial acrylic domes can be disposed of in an
The rooflights upstand is fixed to the roof sub­construction with appropriate landfill. However, due to the value of the materials
screws and brackets (not supplied by VELUX Commercial). The or the carbon content of the wooden and plastic parts, recycling
type of fastening depends on the sub­construction. After fixating or energy recovery is preferable and common.
the upstand, the factory pre­assembled top unit is fixed to the
upstand or ventilation frame using screws. Waste code according to the European Waste List (Regulation
After fixating the complete rooflight, the roof membrane is on the European Waste List):
sealed with materials brought by the installer. 17 02 01 wood
17 02 03 plastics
2.9 Packaging 17 04 02 aluminium
For the transport to the construction site, the VELUX 17 04 05 iron and steel
Commercial acrylic domes are loaded onto a lorry and fixed
2.16 Further information
with multi­use fastening belts. Usually, no additional packaging
is used. Further documentation on the products, technical data sheets,
BIM files, etc. can be found at:
2.10 Condition of use
The material composition of VELUX Commercial acrylic domes www.commercial.velux.com
does not change over their service life.
3. LCA: Calculation rules
A representative acrylic domes in dome shape of the size 850
3.1 Declared Unit mm x 850 mm and with a hight of 300 mm is declared. It
1 m2 of VELUX Commercial acrylic domes is declared. consists of 3­layers of plastic sheets (PC/PMMA/PMMA) and
includes a upstand of insulated wood (48 mm).
Declared unit and mass reference
Name Value Unit 3.2 System boundary
Declared unit 1 m2 Type of the EPD: "cradle to gate with modules C1–C4, and
Grammage 19.80 kg/m2 module D".
3 Environmental Product Declaration ­ VELUX Group ­ VELUX Commercial acrylic dome rooflights (Akrylovenlys)
The production of VELUX Commercial acrylic domes (modules
A1-A3) includes raw material extraction, energy generation, 3.3 Estimates and assumptions
waste treatment and all transports up to the factory gate. In No further assumptions and estimates relevant to the result had
accordance with COUNCIL REGULATION (EU) No 333/2011, to be made beyond the points made in chapter 3 and chapter 4.
secondary metals are modelled as part of the product system
3.4 Cut-off criteria
from the moment they are available as unmixed scrap.
For production wastes that are incinerated, it is as­sumed that No data available from the company survey was neglected.
they are incinerated in a municipal waste incineration plant with These include, among other things, material use, energy
an R­value < 0.6. This means that the incineration process is demand (heat, electricity), packaging materials of raw materials
considered a waste treatment process and included in the cal (insofar as they are generated as waste) and product
culations. The generated 'exported energy' is assumed to have packaging, consumables in production, waste treatment and
reached the end­of­waste status and is considered in module the transport of all inputs and outputs.
D. With this approach, mass and energy flows below 1 % were
also accounted for. No processes were neglected that would
Module A4 is not declared for being optional. In building have been known to the project managers and would have
assessments, the specific transport distance from contributed significantly to the indicators of the impact
Kongerslev/Denmark to the construction site can be assessment.
considered.
3.5 Background data
The products are delivered to the construction site ready to be
Ecoinvent v3.9.1 (2022) with the system model 'allocation – cut­
installed. Minor impacts from installation, e.g. using cranes, etc.
off by classification – unit processes' is used as the background
can be considered insignificant in the light of the total
database.
environmental impacts across the life cycle.
No packaging is used for the transport to the construction site 3.6 Data quality
that would need to be disposed of in module A5. Module A5 is
The foreground data are based on extensive and detailed data
not declared for being optional.
collection at the production site. The foreground data could be
fully linked with corresponding data records from the
Minor impacts from de­installation, e.g. using cranes, etc. can
background database ecoinvent v3.9.1 with the system model
be considered insignificant in the light of the total environmental
"allocation – cut­off by classification – unit processes".
impacts across the life cycle. The values of module C1 are
hence 'zero'.
The background data was updated in 2022. Thus, the quality of
the foreground and background data can be rated as very
In the end­of­life, it is assumed that the disassembled products
good.
are brought to a sorting plant for construction materials, where
The variability of the products consists only in its configuration
metals and burnable wastes are separeted.
(size). An estimate of the variance of results depending on the
size of the products can be found in chapter 7.
Metals a are recycled; it is assumed that these fractions reach
end­of­waste state after having been sorted and transported to 3.7 Period under review
a recycler. Wooden parts and plastics are incinerated (also due The LCA data represents the production conditions for the year
to the very limited data availability on plastics recycling and its 2022.
benefits). On average, an average transport distance of 50 km
has been assumed in module C2 with an average lorry for the 3.8 Geographic Representativeness
transport of the wastes to an incineration plant or to a recycling Land or region, in which the declared product system is
facility. manufactured, used or handled at the end of the product´s
lifespan: Europe
The disassembled product is shredded and the materials are
sorted in module C3. The recovered material leaves the
product system as 'materials for recycling'. The net amounts of 3.9 Allocation
the metals leaving the product system are considered as 'use of No co­products are generated during the production of the
secondary material' in Module D. VELUX Commercial products. Sorted production scrap of the
The wooden parts and the plastics are treated in a waste different metals, notably aluminium, is considered a secondary
incineration plant with an efficiency R1 < 0.6 (according to material with no economic value (so no burdens allocated) and
CEWEP Energy Report III); the recovered energy is reported as considered in the quantification of net flows leaving the product
'exported energy' and considered in Module D. system. This approach is chosen to ensure a coherent
quantification of net flows entering module D.
Module C4 is not declared as a "recovery scenario" is assumed
on product level, including waste treatment from Biogenic carbon is allocated based on physical flows
sorting/recycling in module C3. regardless of the allocation procedure chosen for the process.
The biogenic carbon content of wood products entering or
Module D contains the benefits and loads beyond the system leaving the product system is quantified (manually) as part of
boundary related to the recycling of metals, which result from the GWP in conformity with EN 16485.
the treatment of recycled materials from the point of end­of­
waste status to the point of substitution (as loads) and the No processes were modelled as part of the foreground model
substitution of primary resources (as benefits). that would have required an allocation of multi­input processes.
It also includes the benefits and loads related to the energy Background datasets on municipal waste incineration plants
recovery from plastic and wooden wastes in a municipal waste were taken from ecoinvent without any modification.
incineration plant as modelled in Module C3. Only net flows
leaving the product system are considered in module D. The Allocation of reuse, recycling and recovery was avoided by the
recycled content and the assumed processing losses (e.g., cut­off approach in the foreground model in line with EN 15804.
during remelting) are taken from ecoinvent v.3.9.1 datasets.
4 Environmental Product Declaration ­ VELUX Group ­ VELUX Commercial acrylic dome rooflights (Akrylovenlys)
into account.
3.10 Comparability Ecoinvent v3.9.1 (2022) with the system model 'allocation – cut­
Basically, a comparison or an evaluation of EPD data is only off by classification – unit processes' is used as the background
possible if all the data sets to be compared were created database.
according to EN 15804 and the building context, respectively
the product­specific characteristics of performance, are taken
4. LCA: Scenarios and additional technical information
Module C1
Characteristic product properties of biogenic carbon Inputs and outputs from de­installation are disregared.
Information on describing the biogenic carbon content at
factory gate Module C2
On average, an transport distance of 50 km to a
Note: 1 kg of biogenic carbon is equivalent to 44/12 kg of CO .
2 sorting/recycling facility and an additional 50 km for sorted
Name ValueUnit wooden and plastic parts to a municipal waste incineration
kg plant.
Biogenic carbon content in product ­
C
Biogenic carbon content in accompanying kg Module C3
2.24
packaging C A consumption of 0.03 kWh/kg of electricity for shredding and
sorting and 0.437 MJ/kg of diesel fuel for internal logistics are
• taken into account to disassemble the product. The recovered
material leaves the product system as 'materials for recycling'.
The net amounts of the metals leaving the product system are
considered as 'use of secondary material' in Module D.
Reference service life
Name Value Unit As stated above, it is assumed that 100 % of the wooden and
Life Span according to the plastic parts are treated in a waste incineration plant with an
30 a
manufacturer efficiency R1 < 0.6 (according to CEWEP Energy Report III);
The product has passed according to the same source, an efficiency of 31.0 % is
Declared product internal quality controls and assumed for the production of heat and 18.0 % for the
properties (at the gate) and complies with product ­ production of electricity (always referring to the lower heating
finishes standard for CE marking value of the waste). The recovered energy is reported as
'exported energy' and considered in Module D.
Design application
parameters (if instructed by
Installation according to Module C4
the manufacturer),
assembly instructions and ­ Not relevant according to the assumed end­of­life scenario.
including the references to
state of the art.
the appropriate practices
Module D
and application codes
Module D contains the benefits and loads beyond the system
An assumed quality of
Carried out in accordance boundary related to the recycling of metals, which result from
work, when installed in
with the manufacturer's ­ the treatment of recycled materials from the point of end­of­
accordance with the
instructions. waste status to the point of substitution (as loads) and the
manufacturer’s instructions
substitution of primary resources (as benefits).
Outdoor environment, (for The declared products are It also includes the benefits and loads related to the energy
outdoor applications), e.g. intended for installation recovery from wooden and plastic wastes in a municipal waste
weathering, pollutants, UV outside the building: They are incineration plant as modelled in Module C3.
­
and wind exposure, therefore designed to Only net flows leaving the product system are considered in
building orientation, withstand outdoor conditions module D.
shading, temperature throughout their service life.
Indoor environment (for
The declared products are
indoor applications), e.g.
not intended for installation ­
temperature, moisture,
inside a building.
chemical exposure
Usage conditions, e.g. Standard use in any type of
frequency of use, building, i.e., opening/closing ­
mechanical exposure as often as necessary.
The declared products are
Maintenance e.g. required designed for a reference
frequency, type and quality service life of 30 years. They
­
and replacement of are maintained by cleaning
components water at the discretion of the
building occupants.
5 Environmental Product Declaration ­ VELUX Group ­ VELUX Commercial acrylic dome rooflights (Akrylovenlys)
5. LCA: Results
The set of characterisation factors EF 3.1 has been used.
DESCRIPTION OF THE SYSTEM BOUNDARY (X = INCLUDED IN LCA; MND = MODULE OR INDICATOR NOT DECLARED; MNR
= MODULE NOT RELEVANT)
Benefits and
Construction loads beyond
Product stage Use stage End of life stage
process stage the system
boundaries
la ire ta m w a Ry lp p u s tro p s n a rT g n iru tc a fu n a M e h t m o rf tro p s n a rTe tis e h t o t e ta g y lb m e s s A e s U e c n a n e tn ia M ria p e R tn e m e c a lp e R tn e m h s ib ru fe R y g re n e la n o ita re p Oe s u re ta w la n o ita re p Oe s u n o itc u rts n o c ­e Dn o itilo m e d tro p s n a rT g n is s e c o rp e ts a W la s o p s iD ­e s u e R­y re v o c e R­g n ilc y c e Rla itn e to p
A1 A2 A3 A4 A5 B1 B2 B3 B4 B5 B6 B7 C1 C2 C3 C4 D
X X X MND MND MND MND MNR MNR MNR MND MND X X X X X
RESULTS OF THE LCA - ENVIRONMENTAL IMPACT according to EN 15804+A2: 1 m² of the VELUX Commercial acrylic dome
rooflights
Parameter Unit A1-A3 C1 C2 C3 C4 D
Global Warming Potential total (GWP­total) kg CO 2 eq 7.1E+01 0 2.86E­01 3.94E+01 0 ­6.48E+01
Global Warming Potential fossil fuels (GWP­fossil) kg CO 2 eq 7.97E+01 0 2.86E­01 3.07E+01 0 ­6.04E+01
Global Warming Potential biogenic (GWP­biogenic) kg CO 2 eq ­8.74E+00 0 2.4E­04 8.66E+00 0 ­4.36E+00
Global Warming Potential luluc (GWP­luluc) kg CO 2 eq 8.74E­02 0 1.4E­04 1.17E­03 0 ­9.68E­02
Depletion potential of the stratospheric ozone layer (ODP) kg CFC11 eq 3.47E­06 0 6.27E­09 1.89E­07 0 ­9.6E­07
Acidification potential of land and water (AP) mol H+ eq 3.59E­01 0 1.34E­03 1.77E­02 0 ­1.46E­01
Eutrophication potential aquatic freshwater (EP­freshwater) kg P eq 2.42E­03 0 2.35E­06 6.53E­05 0 ­6.78E­03
Eutrophication potential aquatic marine (EP­marine) kg N eq 6.9E­02 0 5.26E­04 7.78E­03 0 ­2.68E­02
Eutrophication potential terrestrial (EP­terrestrial) mol N eq 8.09E­01 0 5.68E­03 8.52E­02 0 ­3.23E­01
Formation potential of tropospheric ozone photochemical oxidants kg NMVOC
3.08E­01 0 1.98E­03 2.37E­02 0 ­1.04E­01
(POCP) eq
Abiotic depletion potential for non fossil resources (ADPE) kg Sb eq 5.44E­04 0 8.91E­07 3.9E­06 0 ­4.75E­05
Abiotic depletion potential for fossil resources (ADPF) MJ 1.53E+03 0 4.13E+00 2.16E+01 0 ­8.62E+02
m3 world eq
Water use (WDP) 3.19E+01 0 1.8E­02 3.63E­01 0 ­2.69E+00
deprived
RESULTS OF THE LCA - INDICATORS TO DESCRIBE RESOURCE USE according to EN 15804+A2: 1 m² of the VELUX
Commercial acrylic dome rooflights
Parameter Unit A1-A3 C1 C2 C3 C4 D
Renewable primary energy as energy carrier (PERE) MJ 1.64E+02 0 6.43E­02 1.03E+02 0 ­1.37E+02
Renewable primary energy resources as material utilization
MJ 1.02E+02 0 0 ­1.02E+02 0 0
(PERM)
Total use of renewable primary energy resources (PERT) MJ 2.66E+02 0 6.43E­02 1.46E+00 0 ­1.37E+02
Non renewable primary energy as energy carrier (PENRE) MJ 1.15E+03 0 4.13E+00 4.07E+02 0 ­8.76E+02
Non renewable primary energy as material utilization (PENRM) MJ 3.85E+02 0 0 ­3.85E+02 0 0
Total use of non renewable primary energy resources (PENRT) MJ 1.53E+03 0 4.13E+00 2.17E+01 0 ­8.76E+02
Use of secondary material (SM) kg 2.67E­01 0 0 0 0 6.54E­01
Use of renewable secondary fuels (RSF) MJ 0 0 0 0 0 0
Use of non renewable secondary fuels (NRSF) MJ 0 0 0 0 0 0
Use of net fresh water (FW) m3 1.62E+00 0 1.12E­03 2.98E­02 0 ­2.75E­01
RESULTS OF THE LCA – WASTE CATEGORIES AND OUTPUT FLOWS according to EN 15804+A2:
1 m² of the VELUX Commercial acrylic dome rooflights
Parameter Unit A1-A3 C1 C2 C3 C4 D
Hazardous waste disposed (HWD) kg 6.39E­03 0 2.6E­05 1.14E­04 0 ­5.34E­04
Non hazardous waste disposed (NHWD) kg 1.28E+01 0 2.63E­01 1.1E+00 0 ­4.75E+00
Radioactive waste disposed (RWD) kg 4.3E­03 0 2.42E­06 5.73E­05 0 ­5.53E­03
Components for re­use (CRU) kg 0 0 0 0 0 0
Materials for recycling (MFR) kg 5.79E­02 0 0 8.63E­01 0 8.63E­01
Materials for energy recovery (MER) kg 0 0 0 0 0 0
Exported electrical energy (EEE) MJ 3.22E+00 0 0 8.77E+01 0 0
Exported thermal energy (EET) MJ 5.55E+00 0 0 1.51E+02 0 0
RESULTS OF THE LCA – additional impact categories according to EN 15804+A2-optional:
1 m² of the VELUX Commercial acrylic dome rooflights
Parameter Unit A1-A3 C1 C2 C3 C4 D
Disease
Incidence of disease due to PM emissions (PM) 4.15E­06 0 2.81E­08 2.91E­07 0 ­1E­06
incidence
Human exposure efficiency relative to U235 (IR) kBq U235 eq 2.58E+00 0 2.14E­03 3.43E­02 0 ­2.44E+00
6 Environmental Product Declaration ­ VELUX Group ­ VELUX Commercial acrylic dome rooflights (Akrylovenlys)
Comparative toxic unit for ecosystems (ETP­fw) CTUe 2.27E+03 0 2.03E+00 7.98E+01 0 ­1.62E+02
Comparative toxic unit for humans (carcinogenic) (HTP­c) CTUh 1.14E­07 0 1.54E­10 7.65E­09 0 ­1.67E­08
Comparative toxic unit for humans (noncarcinogenic) (HTP­nc) CTUh 9.24E­07 0 3.2E­09 4.65E­08 0 ­2.96E­07
Soil quality index (SQP) SQP 1.31E+03 0 3.1E+00 3.24E+00 0 ­1.05E+02
Disclaimer 1 – for the indicator “Potential Human exposure efficiency relative to U235”. This impact category deals mainly with the
eventual impact of low­dose ionizing radiation on human health of the nuclear fuel cycle. It does not consider effects due to possible
nuclear accidents, occupational exposure or radioactive waste disposal in underground facilities. Potential ionizing radiation from the
soil, radon and from some construction materials is also not measured by this indicator.
Disclaimer 2 – for the indicators “abiotic depletion potential for non­fossil resources”, “abiotic depletion potential for fossil resources”,
“water (user) deprivation potential, deprivation­weighted water consumption”, “potential comparative toxic unit for ecosystems”,
“potential comparative toxic unit for humans – cancerogenic”, “Potential comparative toxic unit for humans ­ not cancerogenic”,
“potential soil quality index”. The results of this environmental impact indicator shall be used with care as the uncertainties on these
results are high as there is limited experience with the indicator.
6. LCA: Interpretation
Figure 1 illustrates the relative contributions of the different dome rooflights.
modules along the life cycle for VELUX Commercial acrylic
Figure 1: Relative environmental impacts of the different The use of renewable primary energy is caused on the one
life cycle stages for VELUX Commercial acrylic dome hand by the share of renewable energy in the electricity mix
rooflights (modules A1–A3 = 100 %) and on the other hand by the primary energy content of sawn
timber and plywood used in the upstand; the production stage
By far the largest part of environmental impacts is caused is the main driver of this impact category whereas the
during production (modules A1­A3) of the VELUX Commercial renewable energy stored in the wooden material is rebooked as
acrylic domes. The contributions of other life cycle stages are used as an energy carrier in module C3.
comparably small.
The use of non­renewable primary energy is mainly caused on
Benefits and burdens beyond the system boundary (module D) the one hand by the share of non­renewable energy in the
are in the order of ­270 % to ­10 % of the impacts over the electricity mix and heat consumption during production and on
product life cycle (modules A1­C4). the other hand by the primary energy content of the plastic
7 Environmental Product Declaration ­ VELUX Group ­ VELUX Commercial acrylic dome rooflights (Akrylovenlys)
materials (polycarbonate and acrylic); the production stage is acrylic/polycarbonate layers, etc.) has been assessed per
the main driver of this impact category whereas the non­ product group. The higher material intensity of the maximum
renewable energy stored in the plastic components is rebooked version is not compensated by a higher surface area covered
as used as an energy carrier in module C3. but lead to higher impact of around 30 % to 50 % in most
impact indicators.
Non­hazardous waste as the quantitatively most relevant waste
flows is mainly caused during maintenance due to the The LCA for the VELUX Commercial products have been
replacement of the motor; hazardous and radioactive waste are calculated for representative products, which are in fact quite
mainly caused by the European electricity mix used during the close to the composition of the weighted average production in
use phase. 2022. To assess the possible variance, a 'maximum' version in
terms of material intensity (highest upstand, highest number of
The LCA for the VELUX Commercial products have been acrylic/polycarbonate layers, etc.) has been assessed per
calculated for representative products, which are in fact quite product group. The higher material intensity of the maximum
close to the composition of the weighted average production in version is not compensated by a higher surface area covered
2022. To assess the possible variance, a 'maximum' version in but lead to higher impact of around 30 % to 50 % in most
terms of material intensity (highest upstand, highest number of impact indicators.
7. Requisite evidence
7.1 Formaldehyde Not applicable; no test defined in applicable product standards.
No test defined in applicable product standards.
7.4 Fire gas toxicity
7.2 MDI No test defined in applicable product standards.
No test defined in applicable product standards.
7.5 VOC emissions
7.3 Checking for pretreatment of the substances used No test defined in applicable product standards.
(Measurement according to AltholzV)
8. References
Product category rules of IBU
ISO 14025
IBU (2021) DIN EN ISO 14025:2006­07, Environmental labels and
IBU 2021): General Instructions for the EPD Programme of the declarations ­ Type III Environmental declarations ­ Principles
Institut Bauen und Umwelt e.V. Version 2.0, Institut Bauen und and procedures.
Umwelt, Berlin.
IBU (2021)
IBU (2021): PCR Part A: Calculation rules for the life cycle
assessment and requirements on the project report according ISO 14044
to EN 15804+A2. Version 1.3, Institut Bauen und Umwelt e.V., DIN EN ISO 14044:2006­07, Environmental management ­ Life
Berlin. cycle assessment ­ Requirements and guidance.
IBU (2023) ECHA candidate list
IBU (2023): PCR Part B: Requirements on the EPD for The candidate list of substances of very high concern,
windows and doors. Version 2023/04, Institut Bauen und European Chemicals Agency, Helsinki. Available at:
Umwelt e.V., Berlin. https://echa.europa.eu/nl/­/four­newsubstances­added­to­the
candidate­list.
Standards and legal documents
Regulation on biocidal products
EN 1873 REGULATION (EU) No 528/2012 OF THE EUROPEAN
EN 1873:2005, Prefabricated accessories for roofing ­ PARLIAMENT AND OF THE COUNCIL of 22 May 2012
Individual rooflights of plastics ­ Product specification and test concerning the making available on the market and use of
methods. biocidal products.
EN 15804 Regulation (EU) Nr. 305/2011(CPR)
DIN EN 15804+A2:2022­03, sustainability of construction REGULATION (EU) No 305/2011 OF THE EUROPEAN
works ­ Environmental product declarations ­ Core rules for the PARLIAMENT AND OF THE COUNCIL of 9 March 2011 laying
product category construction products; German version EN down harmonised conditions for the marketing of construction
15804: 2012+A2:2019 + AC:2021. products and repealing Council Directive 89/106/EEC.
EN 16485 COUNCIL REGULATION (EU) No 333/2011
DIN EN 16485:2014­07, Round and sawn timber ­ COUNCIL REGULATION (EU) No 333/2011 of 31 March 2011
Environmental Product Declarations ­ Product category rules establishing criteria determining when certain types of scrap
for wood and wood­based products for use in construction; metal cease to be waste under Directive 2008/98/EC of the
German version EN 16485:2014. European Parliament and of the Council.
ISO 9001 European Waste List (Waste index)
DIN EN ISO 9001:2015, Quality management systems ­ http://www.gesetze­im­internet.de/avv/anlage.htmEN 16485
Requirements.
8 Environmental Product Declaration ­ VELUX Group ­ VELUX Commercial acrylic dome rooflights (Akrylovenlys)
Additional references (WtE) Plants. CEWEP, Würzburg/Brussels, 2013.
CEWEP Energy Report III ecoinvent v3.9.1
Reimann D.O. (2013): CEWEP Energy Report III (Status 2007 ecoinvent v3.9.1, LCA database, 12/2022. Ecoinvent centre,
– 2010); Results of Specific Data for Energy, R1 Plant Zürich.
Efficiency Factor and NCV of 314 European Waste­to­Energy
9 Environmental Product Declaration ­ VELUX Group ­ VELUX Commercial acrylic dome rooflights (Akrylovenlys)
Publisher
Institut Bauen und Umwelt e.V. +49 (0)30 3087748­ 0
Hegelplatz 1 info@ibu­epd.com
10117 Berlin www.ibu­epd.com
Germany
Programme holder
Institut Bauen und Umwelt e.V. +49 (0)30 3087748­ 0
Hegelplatz 1 info@ibu­epd.com
10117 Berlin www.ibu­epd.com
Germany
Author of the Life Cycle Assessment
Dr. Frank Werner ­ Umwelt & Entwicklung + 41 (0)44 241 39 06
Kammelenbergstrasse 30 frank@frankwerner.ch
9011 St. Gallen http://www.frankwerner.ch/
Switzerland
Owner of the Declaration
VELUX Group +4545164871
Ådalsvej 99 birthe.kjeldsen@velux.com
2970 Hørsholm www.velux.com
Denmark
10 Environmental Product Declaration ­ VELUX Group ­ VELUX Commercial acrylic dome rooflights (Akrylovenlys)
