ENVIRONMENTAL PRODUCT DECLARATION
as per ISO 14025 and EN 15804+A2
Owner of the Declaration dormakaba International Holding GmbH
Publisher Institut Bauen und Umwelt e.V. (IBU)
Programme holder Institut Bauen und Umwelt e.V. (IBU)
Declaration number EPD-DOR-20220168-CBA5-EN
Issue date 18.10.2022
Valid to 17.10.2027
Cencon ATM Cash Vault Security System
dormakaba
www.ibu-epd.com | https://epd-online.com
General Information
dormakaba Cencon ATM Cash Vault Security System
Programme holder Owner of the declaration
IBU – Institut Bauen und Umwelt e.V. dormakaba International Holding GmbH
Hegelplatz 1 DORMA Platz 1
10117 Berlin 58256 Ennepetal
Germany Germany
Declaration number Declared product / declared unit
EPD-DOR-20220168-CBA5-EN 1 Cencon ATM Cash Vault Security System (1piece), consisting of the
following items:
- Cencon ATM lock
- product packaging
This declaration is based on the product category rules: Scope:
Electronic and physical Access Control Systems, 01.08.2021 This declaration is a specific product declaration for the Cencon ATM Cash
(PCR checked and approved by the SVR) Vault Security System.
The underlying life cycle assessment is based on the entire life cycle of
this specific Cencon ATM Cash Vault Security System manufactured by
Issue date dormakaba. The various technical features are outlined in chapter 2. The
products are manufactured at the dormakaba production facility in Nogales
18.10.2022
(Mexico).
The year of data collection is 2021. The declared product is a self-powered
solution.
Valid to
The owner of the declaration shall be liable for the underlying information
17.10.2027 and evidence; the IBU shall not be liable with respect to manufacturer
information, life cycle assessment data and evidences.
The EPD was created according to the specifications of EN 15804+A2. In
the following, the standard will be simplified as EN 15804.
Verification
The standard EN 15804 serves as the core PCR
Independent verification of the declaration and data according to ISO
14025:2011
internally X externally
Dipl.-Ing. Hans Peters
(Chairman of Institut Bauen und Umwelt e.V.)
Florian Pronold Dr.-Ing. Wolfram Trinius,
(Managing Director Institut Bauen und Umwelt e.V.) (Independent verifier)
1 Environmental Product Declaration - dormakaba - Cencon ATM Cash Vault Security System
Product
• Key: Up to 32 events
Product description/Product definition • Software: Unlimited events
The Cencon ATM Cash Vault Security System from dormakaba • Time Windows: by User Optional
is designed to combat insider theft from ATMs through the • Time Delay: 1-99 minutes, Bank mode only
combined use of lock hardware, systems software and Smart • Number of Users: Unlimited for FLM & Route mode,
Keys™. Cencon offers total access control and accountability 100 per lock for Bank mode
with its One Time Combination™ feature. The One Time
Combination is dispatched from a central location and cannot Alarm Interface
be reused at a later date, thus eliminating temptation. • Silent Duress Alarm: Standard – combination +10
• Bolt Status: Standard
Unique software allows you to control and monitor nearly • Alarm Shunt: Optional The products are not harmonised in
unlimited numbers of locks located anywhere in the world - from accordance with the Construction Product Regulations (CPR)
one central location. Cencon is a solution to today's most but in accordance with other provisions for harmonisation of the
serious security challenges. EU.
• Cencon and CenTran system supporting software Compliance with the European Union Directive and technical
• Three independent operating modes in one lock specifications:
• Unlimited Cencon system users/100 Bank Mode users • DIN EN 1300: 2019-05, Secure storage units -
• One Time Combination for FLM and CIT (Route) users Classification for high security locks
• Dead bolt or Swing bolt available according to their resistance to unauthorized opening.
• EN 1300 B, VdS class 2, SBSC, UL type 1 The products are subject to CE marking according to the
For placing the Cencon ATM Cash Vault Security System on relevant harmonization legislation.
the market in the European Union/European Free Trade
Association (EU/EFTA) (with the exception of Switzerland) the
following legal provisions apply: Base materials/Ancillary materials
Performance data of the product with respect to its
characteristics in accordance with the relevant technical
• VdS 2344:2014-07
provision which can be applied are mentioned above.
• VdS 2396:2014-07
The major material composition including packaging is listed
• UL 2058:2005-06
below:
• DIN EN1300:2019-05
• Restriction of Hazardous Substances (RoHS)
Application
The Cencon Locks can work individually and give shared
access.
Three modes are available
1 FLM Mode: For the First Line Maintenance personnel.
2. Route Mode: For cash replenisher or armored service.
3. Bank Mode: For bank branch employees.
Each mode addresses the individual access needs for each
category of user.
Technical Data
Access Control The product includes partial articles which contain substances
• User Authentication: Combination + Smart Key listed in the Candidate List of REACH Regulation
• Operating Modes: Three Modes (FLM, Route and Bank) 1907/2006/EC (date: 14.06.2023) exceeding 0.1 percentage by
• Single or Dual User Access: For any of the three modes mass: no
• Factory (Shelved) Mode: 50-25-50 or changeable by user
• One Time Combination: For FLM & Route Mode The Candidate List can be found on the ECHA website
• User-Defined Combinations: For Bank Mode users address: https:echa.europs.eu/de/home.
• Wrong Combo Penalty: After five incorrect attempts
• Central Control: With Cencon 5 software Reference service life
The product is certified according to UL 2058 with testing up to
Audit Trail: 25.000 cycles. Under normal conditions and depending on
• Lock: Can achieve more than 1,000 events cycle frequency, it means an approximate duration of 7 years.'
LCA: Calculation rules
Name Value Unit
Declared Unit
Declared unit 1 pce.
The declared unit is 1 piece of the product: 0.982kg without
Mass (total system) 0.982 kg
packaging
System boundary
2 Environmental Product Declaration - dormakaba - Cencon ATM Cash Vault Security System
The type of EPD is: cradle to gate with options, modules C1– — C1, de-construction, demolition:
C4, and module D (A1–A3 + C + D and additional modules: A4 — C2, transport to waste processing;
+ A5 + B6) — C3, waste processing for reuse, recovery and/or recycling;
— C4, disposal;
Production - Module A1-A3 including provision and all transport, provision of all materials,
The product stage includes: products and related energy and water use.
— A1, raw material extraction, processing and mechanical
treatments, processing of secondary material input (e.g. Module D (Benefits and loads beyond the system boundary)
recycling processes), includes:
— A2, transport to the manufacturer, — D, recycling potentials, expressed as net impacts and
— A3, manufacturing and assembly including provision of all benefits.
materials, products and energy, as well as waste processing up
to the end-of waste state. Geographic Representativeness
Land or region, in which the declared product system is
Construction stage - Modules A4-A5 manufactured, used or handled at the end of the product´s
The construction process stage includes: lifespan: United States
— A4, transport to the building site;
— A5, installation into the building;
Comparability
including provision of all materials, products and energy, as well
Basically, a comparison or an evaluation of EPD data is only
as waste processing up to the end-of-waste state or disposal of
possible if all the data sets to be compared were created
final residues during the construction process stage.
according to EN 15804 and the building context, respectively
the product-specific characteristics of performance, are taken
End-of-life stage– Modules C1-C4 and D
into account.
The end-of-life stage includes:
LCA: Scenarios and additional technical information
Reference service life
Characteristic product properties of biogenic carbon
Name Value Unit
Information on describing the biogenic Carbon Content at
Life Span according to the manufacturer 7 a
factory gate
Name ValueUnit
kg
Biogenic carbon content in product -
C End of life (C1-C4)
Biogenic carbon content in accompanying kg C1: The product dismantling from the building is done manually
0.01
packaging C without environmental burden.
C2: Transport to waste treatment at end of life is 50km.
Name Value Unit
Collected separately waste type waste type 0.982 kg
Transport to the building site (A4)
Reuse - kg
Name Value Unit
Recycling 0.613 kg
Litres of fuel 0.00276l/100km
Energy recovery 0.331 kg
Capacity utilisation (including empty runs) via
55 % Landfilling 0.038 kg
medium truck
Transport to waste management 50 km
Transport distance via medium truck 100 km
Transport distance via plane 2800 km The product is disassembled in a recycling process. Material
recycling is then assumed for the metals, electronic and
The product is transported via truck and plane. The main
electromechanics. The plastic components are assumed to be
distribution regions are Mexico and US with the calculated
incinerated with energy recovery. Minor proportions of residues
average transport distances.
arising from the recycling process are landfilled. Region for the
End of Life is: Global.
Installation into the building (A5)
Name Value Unit Reuse, recovery and/or recycling potentials (D), relevant
scenario information
Waste plastics 0.000017 kg
Collection rate is 100 %.
Waste paper 0,00005 kg
3 Environmental Product Declaration - dormakaba - Cencon ATM Cash Vault Security System
LCA: Results
DESCRIPTION OF THE SYSTEM BOUNDARY (X = INCLUDED IN LCA; MND = MODULE OR INDICATOR NOT DECLARED; MNR
= MODULE NOT RELEVANT)
Benefits and
Construction loads beyond
Product stage Use stage End of life stage
process stage the system
boundaries
la ire ta m w a Ry lp p u s tro p s n a rT g n iru tc a fu n a M e h t m o rf tro p s n a rTe tis e h t o t e ta g y lb m e s s A e s U e c n a n e tn ia M ria p e R tn e m e c a lp e R tn e m h s ib ru fe R y g re n e la n o ita re p Oe s u re ta w la n o ita re p Oe s u n o itc u rts n o c -e Dn o itilo m e d tro p s n a rT g n is s e c o rp e ts a W la s o p s iD -e s u e R-y re v o c e R-g n ilc y c e Rla itn e to p
A1 A2 A3 A4 A5 B1 B2 B3 B4 B5 B6 B7 C1 C2 C3 C4 D
X X X X X MND MND MNR MNR MNR MND MND MND X X X X
RESULTS OF THE LCA - ENVIRONMENTAL IMPACT according to EN 15804+A2: 1 piece CENCON
Parameter Unit A1-A3 A4 A5 C2 C3 C4 D
GWP-total kg CO 2 eq 1.59E+01 1.72E+00 2.6E-02 4E-03 8.41E-01 7.6E-04 -6.8E+00
GWP-fossil kg CO 2 eq 1.59E+01 1.71E+00 4E-03 4E-03 8.41E-01 7.55E-04 -6.78E+00
GWP-biogenic kg CO 2 eq 2.5E-02 3E-03 2.1E-02 1.85E-04 1.96E-05 2.58E-06 -1.4E-02
GWP-luluc kg CO 2 eq 1.11E-02 3.58E-05 5.7E-07 9.54E-08 4.76E-05 2.17E-06 -3E-03
ODP kg CFC11 eq 3.58E-10 1.25E-16 5.82E-18 4.23E-19 4.24E-16 2.8E-18 -2.15E-14
AP mol H+ eq 1.12E-01 7E-03 6.81E-06 4.01E-06 1.5E-04 5.42E-06 -6.7E-02
EP-freshwater kg P eq 3.52E-05 2.8E-07 1.07E-09 8.58E-10 6.77E-08 1.3E-09 -5.9E-06
EP-marine kg N eq 1.77E-02 3E-03 2.37E-06 1.28E-06 3.38E-05 1.39E-06 -1E-02
EP-terrestrial mol N eq 1.91E-01 3.4E-02 3.07E-05 1.42E-05 6.82E-04 1.53E-05 -1.14E-01
kg NMVOC
POCP 5.17E-02 9E-03 6.3E-06 3.61E-06 9.35E-05 4.22E-06 -3.1E-02
eq
ADPE kg Sb eq 6E-03 4.85E-08 8.81E-11 1.2E-10 5.82E-09 6.78E-11 -5E-03
ADPF MJ 2.21E+02 2.32E+01 9E-03 5.7E-02 3.9E-01 1E-02 -7.66E+01
m3 world eq
WDP 4.01E+00 3E-03 3E-03 7.86E-06 8.6E-02 7.91E-05 -1.01E+00
deprived
GWP = Global warming potential; ODP = Depletion potential of the stratospheric ozone layer; AP = Acidification potential of land and water; EP =
Eutrophication potential; POCP = Formation potential of tropospheric ozone photochemical oxidants; ADPE = Abiotic depletion potential for non-fossil
resources; ADPF = Abiotic depletion potential for fossil resources; WDP = Water (user) deprivation potential)
RESULTS OF THE LCA - INDICATORS TO DESCRIBE RESOURCE USE according to EN 15804+A2: 1 piece CENCON
Parameter Unit A1-A3 A4 A5 C2 C3 C4 D
PERE MJ 3.54E+01 5.6E-02 1.88E-01 1.79E-04 1.01E-01 1E-03 -8.89E+00
PERM MJ 1.86E-01 0 -1.86E-01 0 0 0 0
PERT MJ 3.56E+01 5.6E-02 2E-03 1.79E-04 1.01E-01 1E-03 -8.89E+00
PENRE MJ 2.1E+02 2.33E+01 7.1E-02 5.7E-02 1.14E+01 1E-02 -7.67E+01
PENRM MJ 1.11E+01 0 -6.2E-02 0 -1.1E+01 0 0
PENRT MJ 2.22E+02 2.33E+01 9E-03 5.7E-02 3.9E-01 1E-02 -7.67E+01
SM kg 4.5E-02 0 0 0 0 0 0
RSF MJ 0 0 0 0 0 0 0
NRSF MJ 0 0 0 0 0 0 0
FW m3 1.11E-01 1.09E-04 7.32E-05 3.22E-07 2E-03 2.5E-06 -3E-02
PERE = Use of renewable primary energy excluding renewable primary energy resources used as raw materials; PERM = Use of renewable primary
energy resources used as raw materials; PERT = Total use of renewable primary energy resources; PENRE = Use of non-renewable primary energy
excluding non-renewable primary energy resources used as raw materials; PENRM = Use of non-renewable primary energy resources used as raw
materials; PENRT = Total use of non-renewable primary energy resources; SM = Use of secondary material; RSF = Use of renewable secondary fuels;
NRSF = Use of non-renewable secondary fuels; FW = Use of net fresh water
RESULTS OF THE LCA – WASTE CATEGORIES AND OUTPUT FLOWS according to EN 15804+A2:
1 piece CENCON
Parameter Unit A1-A3 A4 A5 C2 C3 C4 D
HWD kg 3.06E-06 2.22E-09 1.67E-11 5.52E-12 1.49E-09 1.51E-10 -7.25E-07
NHWD kg 4.03E-01 2E-03 1E-03 5.82E-06 8.7E-02 5E-02 6.1E-02
RWD kg 8.07E-03 1.91E-05 4.28E-07 6.11E-08 1.45E-05 1.13E-07 -2E-03
CRU kg 0 0 0 0 0 0 0
MFR kg 0 0 0 0 6E-01 0 0
MER kg 0 0 0 0 0 0 0
EEE MJ 1.07E-04 0 4E-02 0 0 0 0
EET MJ 1.95E-04 0 7.6E-02 0 0 0 0
HWD = Hazardous waste disposed; NHWD = Non-hazardous waste disposed; RWD = Radioactive waste disposed; CRU = Components for re-use;
MFR = Materials for recycling; MER = Materials for energy recovery; EEE = Exported electrical energy; EET = Exported thermal energy
4 Environmental Product Declaration - dormakaba - Cencon ATM Cash Vault Security System
RESULTS OF THE LCA – additional impact categories according to EN 15804+A2-optional:
1 piece CENCON
Parameter Unit A1-A3 A4 A5 C2 C3 C4 D
Disease
PM 1.06E-06 2.25E-08 4.25E-11 2.11E-11 1.91E-09 6.71E-11 -6.05E-07
incidence
IR kBq U235 eq 8.29E-01 3E-03 6.21E-05 8.73E-06 1E-03 1.16E-05 -2.45E-01
ETP-fw CTUe 1.2E+02 1.65E+01 4E-03 4E-02 1.46E-01 6E-03 -1.88E+01
HTP-c CTUh 5.46E-08 3.1E-10 2.3E-13 7.58E-13 1.27E-11 8.39E-13 5.4E-09
HTP-nc CTUh 3.98E-07 1.43E-08 1.32E-11 3.24E-11 1.28E-09 9.24E-11 6.89E-07
SQP SQP 4.37E+01 4.7E-02 2E-03 1.46E-04 1.17E-01 2E-03 -4.27E+00
PM = Potential incidence of disease due to PM emissions; IR = Potential Human exposure efficiency relative to U235; ETP-fw = Potential comparative
Toxic Unit for ecosystems; HTP-c = Potential comparative Toxic Unit for humans (cancerogenic); HTP-nc = Potential comparative Toxic Unit for humans
(not cancerogenic); SQP = Potential soil quality index
Disclaimer 1 – for the indicator IRP
This impact category deals mainly with the eventual impact of low dose ionizing radiation on human health of the nuclear fuel cycle. It
does not consider effects due to possible nuclear accidents, occupational exposure nor radioactive waste disposal in underground
facilities. Potential ionizing radiation from the soil, from radon and from some construction materials is also not measured by this
indicator.
Disclaimer 2 – for the indicators ADPE, ADPF, WDP, ETP-fw, HTP-c, HTP-nc, SQP
The results of this environmental impact indicator shall be used with care as the uncertainties on these results are high or as there is
limited experienced with the indicator.
References
DIN EN 1300 Directive (EU) No 2011/65.
DIN EN 1300:2019, Secure storage units - Classification for
high security locks according to their resistance to unauthorized European Chemicals Agency (ECHA)
opening https://echa.europa.eu/de/
DIN EN ISO 14025: Further References
DIN EN ISO 14025:2011-10, Environmental labels and
declarations — Type III environmental declarations - Principles IBU 2021
and procedures. General Instructions for the EPD programme of Institut Bauen
und Umwelt e.V. Version 2.0, Berlin: Institut Bauen und Umwelt
EN 15804:2019+A2 e.V., 2021. www.ibu-epd.com
EN 15804+A2:2019+AC:2021, Sustainability of construction
works — Environmental Product Declarations — Core rules for GaBi ts software
the product category of construction products. Sphera Solutions GmbH Gabi Software System and Database
for Life Cycle Engineering 1992-2020 Version 10.0.0.71
UL 2058 University of Stuttgart Leinfelden-Echterdingen
UL 2058: 2005-06,Underwriters Laboratories, High-Security
Electronic locks GaBi ts documentation
GaBi life cycle inventory data documentation (https://www.gabi-
VdS 2344 software.com/support/gabi/gabidatabase- 2020-lci-
VdS 2344:2014-07, Procedure for the testing, approval and documentation/).
certification of products and systems for fire protection and
security technologies LCA-tool dormakaba
LCA tool SAL No.:
VdS 2396 IBU-DOR-IBU-DOR-202105-LT1-EN Developed by Sphera
VdS 2396:2014-07, VdS Guidelines for Physical Security Solutions GmbH.
Devices - High Security Locks for Secure Storage Units -
Requirements and Test Methods PCR Part A
PCR – Part A: Calculation Rules for the Life Cycle Assessment
Registration, Evaluation, Authorisation and Restriction of and Requirements on the Project Re-port according to EN
Chemicals (REACH) 15804+A2:2019, Version 1.0, Institut Bauen und Umwelt e.V.,
Regulation (EC) No 1907/2006 of the European Parliament and www.ibu-epd.com.
of the Council on the Registration, Evaluation, Authorisation
and Restriction of Chemicals (REACH). PCR Part B
PCR – Part B: Requirements on the EPD for Electronic and
Restriction of Hazardous Substances (RoHS) physical Access Control Systems, version 08/2021, Institut
Directive on the restriction of the use of certain hazardous Bauen und Umwelt e.V., www.ibu-epd.com.
substances in electrical and electronic equipment (RoHS),
5 Environmental Product Declaration - dormakaba - Cencon ATM Cash Vault Security System
Publisher
Institut Bauen und Umwelt e.V. +49 (0)30 3087748- 0
Hegelplatz 1 info@ibu-epd.com
10117 Berlin www.ibu-epd.com
Germany
Programme holder
Institut Bauen und Umwelt e.V. +49 (0)30 3087748- 0
Hegelplatz 1 info@ibu-epd.com
10117 Berlin www.ibu-epd.com
Germany
Author of the Life Cycle Assessment
Sphera Solutions GmbH +49 711 341817-0
Hauptstraße 111- 113 info@sphera.com
70771 Leinfelden-Echterdingen www.sphera.com
Germany
Owner of the Declaration
dormakaba International Holding GmbH +49 2333 793-0
DORMA Platz 1 info.de@dormakaba.com
58256 Ennepetal www.dormakaba.com
Germany
6 Environmental Product Declaration - dormakaba - Cencon ATM Cash Vault Security System
