ENVIRONMENTAL PRODUCT DECLARATION
as per ISO 14025 and EN 15804+A2
Owner of the Declaration DuPont de Nemours (Luxembourg) s.à r.l.
Programme holder Institut Bauen und Umwelt e.V. (IBU)
Publisher Institut Bauen und Umwelt e.V. (IBU)
Declaration number EPD-DUP-20210186-IBC1-EN
Issue date 30.11.2021
Valid to 29.11.2026
DuPont™ Tyvek® 2506B
DuPont de Nemours (Luxembourg) s.à r.l.
www.ibu-epd.com | https://epd-online.com
Umwelt Produktdeklaration Name des Herstellers – Name des Produkts
1. General Information
DuPont de Nemours (Luxembourg) s.à r.l. DuPont™ Tyvek® 2506B
Programme holder Owner of the declaration
IBU – Institut Bauen und Umwelt e.V. DuPont de Nemours (Luxembourg) s.à r.l.
Panoramastr. 1 Rue Général Patton
10178 Berlin L-2984 Contern
Germany Luxembourg
Declaration number Declared product / declared unit
EPD-DUP-20210186-IBC1-EN 1 m² DuPont™ Tyvek® 2506B
This declaration is based on the product Scope:
category rules: This document applies to DuPont™ Tyvek® 2506B, a
False ceiling and underlay sheeting, 11.2017 laminated high density polyethylene (HDPE)
(PCR checked and approved by the SVR) membrane manufactured by DuPont in L-2984 Contern
and laminated as well as printed in Germany, with
a declared unit weight of 148 g/m2. The LCA data were
Issue date
compiled using production data from the year 2019
30.11.2021
by DuPont. The declaration holder is responsible for
the underlying data and its verification.
Valid to
29.11.2026
The owner of the declaration shall be liable for the
underlying information and evidence; the IBU shall not
be liable with respect to manufacturer information, life
cycle assessment data and evidences.
The EPD was created according to the specifications
of EN 15804+A2. In the following, the standard will be
simplified as EN 15804.
Verification
The standard EN 15804 serves as the core PCR
Independent verification of the declaration and data
according to ISO 14025:2010
Dipl. Ing. Hans Peters internally x externally
(chairman of Institut Bauen und Umwelt e.V.)
Dr. Alexander Röder Vito D'Incognito
(Managing Director Institut Bauen und Umwelt e.V.)) (Independent verifier)
2. Product
2.1 Product description/Product definition installed below Tyvek® is kept dry and performs as
DuPont™ Tyvek® is a nonwoven material made of designed.
HDPE, which is diffusion open but watertight. It is used
as a roof and wall underlay.
For the placing on the market of the product in the 2.3 Technical Data
European Union/European Free Trade Association The following chapter comprises technical data for the
(EU/EFTA) (with the exception of Switzerland) characteristics listed in the Declaration of Performance
Regulation (EU) No. 305/2011 (CPR) applies. The according to the harmonized technical specifications
product needs a declaration of performance taking into EN 13859-1 and EN 13859-2.
consideration EN 13859-1:2010 Flexible sheets for
waterproofing - Definitions and characteristics of Technical Data
underlays - Part 1: Underlays for discontinuous roofing Name Value Unit
and EN 13859-2:2010 Flexible sheets for 50m
Length acc. to EN 1848-2 m
waterproofing - Definitions and characteristics of standard
underlays - Part 2 Underlays for walls and the CE- 1.5m
Width acc. to EN 1848-2 m
marking. For the application and use the respective standard
national provisions apply. Grammage acc. to EN 1849-2 0.148 kg/m2
2.2 Application Resistance to water penetration
W1 -
Tyvek® underlays are used in roofs and walls. They acc. to EN 1928 (class)
constitute the second water shedding layer and at the Water vapor diffusion equivalent
same time protect the insulation from trapped air layer thickness acc. to EN ISO 0.03 m
moisture, wind penetration, dust and insects. Insulation 12572
2 Environmental Product Declaration DuPont de Nemours (Luxembourg) s.à r.l. – Tyvek® 2506B
Maximum tensile force acc. to EN fix it to the construction. Refer to Tyvek® installation
340/280 N/50mm
12311-1 guidelines for more information.
Elongation acc. to EN 12311-1 12/18,5 %
Resistance to water penetration 2.9 Packaging
after ageing acc. to EN 1297, EN W1 - Tyvek® is wound onto carton cores. Each roll comes
1928 (class) with a paper insert sheet. Rolls are individually
Tear resistance (nail) acc. to EN wrapped in foil (LDPE: low density PE) and stacked on
165/175 N
12310-1 wooden pallets which are also wrapped in LDPE
stretch film. Vertical sides of the pallets are protected
with a carton profile.
Performance data of the product in accordance with All packaging materials can be reused (e.g. pallets),
the declaration of performance with respect to its recycled or valorised through energy recovery.
essential characteristics according to EN 13859-
1:2010 Flexible sheets for waterproofing - Definitions
and characteristics of underlays - Part 1: Underlays for 2.10 Condition of use
discontinuous roofing and EN 13859-2:2010 Flexible Materials are not expected to change or react during
sheets for waterproofing - Definitions and the period of use. Tyvek® is intended to be installed on
characteristics of underlays - Part 2 Underlays for walls the cold side of the building envelope and is designed
to withstand substantial temperature changes during
2.4 Delivery status service life.
The single selling unit is a roll of up to 3 m width and a
length of up to 100 m. Usually several rolls are 2.11 Environment and health during use
strapped and piled on a wooden pallet. Tyvek® membranes are usually concealed below roof
The order unit is square meter [m²]. decking or facade cladding. They do not require
maintenance and will not produce emissions. There
2.5 Base materials/Ancillary materials are no environmental or health concerns to be
Tyvek® 2506B is a laminate of a high density expected from the use of the material.
polyethylene (HDPE) nonwoven (functional layer) and
a polypropylene (PP) spunbond. Both materials are 2.12 Reference service life
glued during the lamination process. Both the PP and The documentation of the RSL is not required for this
the HDPE are UV stabilized with hindered amine light EPD since not the entire life cycle is declared (without
stabilizers (HALS). modules B1-B7). Nevertheless, the product is
Concentrations: assumed to have a reference service life of 30 years,
2506B corresponding to the average roof lifetime (BNB
Tyvek® HDPE nonwoven 55 % Nutzungsdauerliste). But this assumption could not be
Spunbond PP 34 % verified because the Tyvek® envelopes have only
Adhesive 10 % been sold for 25 years.
HALS < 1 %
2.13 Extraordinary effects
2.6 Manufacture
Tyvek® underlays are produced on semi-continuously Fire
operating production facilities in different countries.
Process steps include:
1. Spinning of thin HDPE filaments. Fire protection
2. Bonding of filament sheet. Name Value
3. Laminating of a spunbond onto the Tyvek® sheet. Building material class acc. to E
4. Printing, slitting and packaging of the finished roll EN13501-1
goods.
Water
2.7 Environment and health during Tyvek® membranes are inherently waterproof. No part
manufacturing of the product will dissolve in water nor will the product
Some of the manufacturing facilities employed in the release any toxic substances to water.
production of Tyvek® are ISO 14001 certified. All
facilities comply with local regulations and DuPont Mechanical destruction
internal standards. No possible impacts on the environment following
Particular care is taken to ensure the safety of anyone unforeseeable mechanical destruction are known.
involved in the Tyvek® supply chain in line with the
DuPont safety culture: all injuries can be prevented 2.14 Re-use phase
(goal is ZERO). The material is not intended to be re-used or recycled.
Energy recovery is possible.
2.8 Product processing/Installation
Tyvek® membranes for walls and roofs can be either 2.15 Disposal
installed on the construction site or in manufacturing Disposal of the material should be made according to
facilities in case of pre-fabricated buildings. In both national legislation. Incineration is the preferred way of
instances the material is usually installed by manually disposal. European Waste Codes (Commission
unwinding the sheet from the roll and placing it onto decision 2014/955/EU) for mixed construction and
the designated surface. Tools required are usually a demolition waste is 17 09 04.
knife or scissors to cut the sheet as well as a stapler to
3 Environmental Product Declaration DuPont de Nemours (Luxembourg) s.à r.l. – Tyvek® 2506B
2.16 Further information
Additional information about product properties and
use can be found at www.building.dupont.com.Safety
Data Sheets (SDS) or Article Information Sheets (AIS)
of the products can be found at www.dupont.com.
3. LCA: Calculation rules
3.1 Declared Unit of missing data, a cut-off criteria of 1 % of the total
This declaration applies to 1 m2 of DuPont™ Tyvek® input mass was applied for unit processes and 5 % for
2506B membrane, with a declared unit weight of 148 the entire modules (as recommended by EN 15804,
g/m2. section 6.3.5) and therefore some inputs were
excluded: tape and spiking agent for monolayer
Declared Unit production (sum < 0.04 % of total input mass for
Name Value Unit monolayer production), paper ink, hotmelt, paper, tape
Declared unit 1 m2 and detergent for finishing process (sum < 0.2 % of
Grammage 0.148 kg/m2 total input mass for finishing process). Transports were
considered for all inputs and outputs. Manufacturing of
the production machines and systems and associated
infrastructure were not taken into account in the life
3.2 System boundary cycle assessment (LCA). Regarding possible off-cuts
Type of EPD: Cradle-to-gate (with options) during installation, the amount is lower than 5 % and
The system boundaries of the EPD follow the modular therefore also neglected.
construction system as described by EN 15804. The
LCA takes into account the following modules: 3.5 Background data
 A1-A3: Manufacturing of pre-products, All background data for the LCA model were taken
from the database of GaBi 10.5.0.78.
packaging, ancillary materials, transport to the
factory, production including energy supply
3.6 Data quality
and waste handling
To simulate the product stage, data recorded by
 A4: Transport to the construction site DuPont Luxembourg s.à r.l. and the lamination and the
 A5: Installation into the building (disposal of converting plants in Germany from the production year
packaging) 2019 were used.
Eurostat data for the years 2018-2019 were used to
 C4: Waste disposal (incineration)
model the modules A4 (freight transport modal split)
 D: Potential for reuse, recovery and/or
and A5 (packaging disposal routes).
recycling (benefits for incineration and Regarding background processes, the Luxembourg
recovery of packaging materials from module and German electricity grid mix were applied to the
A5 and envelopes incineration from module production plants in these countries (A1-A3). Other
C4). background data were specific to Germany or the
European average, and were not older than than10
years.
The representativeness can be classified as very good
3.3 Estimates and assumptions
for all the foreground data, and most of the background
The spunbond polypropylene (SBPP) production was
data.
modelled considering the consumption of
polypropylene granulates and the following
3.7 Period under review
assumptions:
The period of study encompasses the year 2019.
 material loss of 5% during the bonding
process (1.05 kg of granulates are finally 3.8 Allocation
used to produce 1 kg of SBPP); Mass allocation was applied for production. At the
 consumption of electricity based on supplier DuPont site in Luxembourg, Tyvek® waste materials
are sold and transformed externally. The further use of
data (1-1.2 kWh per kg of produced
the valorized HDPE granulates was cut-off from the
nonwoven) which has been adapted to
system boundaries, as for the packaging materials
account for the older technology (1.5 kWh per
sent for recycling. The Tyvek® final waste material
kg of SBPP). sent to incineration is modelled through the
combustion process of the specific material and the
avoided conventional energy production is considered
The polypropylene (PP) loss of 0.05 kg per 1 kg of
in module D. The potential benefit in module D will be
SBPP was assumed to be incinerated.
possible only if the Tyvek® will be separate and
incinerated.
The colour paste used in the finishing process was
valued with a general composition of water-based
3.9 Comparability
colour paste (conservative approach).
Basically, a comparison or an evaluation of EPD data
is only possible if all the data sets to be compared
3.4 Cut-off criteria
were created according to EN 15804 and the building
All data were taken into consideration (recipe
constituents, process water, electricity used). In case
4 Environmental Product Declaration DuPont de Nemours (Luxembourg) s.à r.l. – Tyvek® 2506B
context, respectively the product-specific
characteristics of performance, are taken into account.
GaBi 10.5.0.78 was used to model background data.
5 Environmental Product Declaration DuPont de Nemours (Luxembourg) s.à r.l. – Tyvek® 2506B
4. LCA: Scenarios and additional technical information
Characteristic product properties
Information on biogenic Carbon
The product does not contain biogenic carbon.
Information on describing the biogenic Carbon
Content at factory gate
Name Value Unit
Biogenic Carbon Content in
0 kg C
product
Biogenic Carbon Content in
0.0037 kg C
accompanying packaging
The following technical information serves as a basis
for the declared modules or can be used for the
development of specific scenarios in the context of a
building assessment.
Transport from the gate to the construction site
(A4)
Name Value Unit
Transport distance (weighted
3064 km
average)
Transport (train) 3.64E-02 tkm
Transport (road) 1.58E-01 tkm
Transport (water) 2.93E-01 tkm
Installation of the product into the building (A5)
Name Value Unit
Wood waste to landfill 2.97E-04 kg
Wood waste to incineration 1.78E-04 kg
Cardboard waste to landfill 2.96E-04 kg
Cardboard waste to incineration 2.26E-04 kg
Plastic waste to landfill 2.66E-05 kg
Plastic waste to incineration 3.63E-05 kg
In case a reference service life according to
applicable ISO standards is declared then the
assumptions and in-use conditions underlying the
determined RSL shall be declared. In addition, it shall
be stated that the RSL applies for the reference
conditions only
The same holds for a service life declared by the
manufacturer. Corresponding information related to in-
use conditions needs not be provided if a service life
taken from the list on service life by BNB is declared.
End-of-life stage (C1-C4)
Name Value Unit
Collected separately Tyvek® waste 0.148 kg
Energy recovery 100 %
R1 value < 0.6
6 Environmental Product Declaration DuPont de Nemours (Luxembourg) s.à r.l. – Tyvek® 2506B
5. LCA: Results
The results displayed below apply to 1 m2 of DuPont™ Tyvek® 2506B membrane, with a declared unit weight of
148 g/m2.
Disclaimers:
Potential Human exposure efficiency relative to U235: This impact category deals mainly with the eventual impact
of low dose ionizing radiation on human health of the nuclear fuel cycle. It does not consider effects due to
possible nuclear accidents, occupational exposure nor due to radioactive waste disposal in underground facilities.
Potential ionizing radiation from the soil, from radon and from some construction materials is also not measured
by this indicator.
Abiotic depletion potential for non-fossil resources; Abiotic depletion potential for fossil resources; Water (user)
deprivation potential, deprivation-weighted water consumption: The results of these environmental impact
indicators shall be used with care as the uncertainties on these results are high or as there is limited experienced
with the indicator.
Disclaimer:
EP-freshwater: This indicator has been calculated as “kg P eq” as required in the characterization model
(EUTREND model, Struijs et al., 2009b, as implemented in ReCiPe;
http://eplca.jrc.ec.europa.eu/LCDN/developerEF.xhtml).
DESCRIPTION OF THE SYSTEM BOUNDARY (X = INCLUDED IN LCA; ND = MODULE OR INDICATOR NOT
DECLARED; MNR = MODULE NOT RELEVANT)
BENEFITS AND
CONSTRUCTI LOADS
PRODUCT STAGE ON PROCESS USE STAGE END OF LIFE STAGE BEYOND THE
STAGE SYSTEM
BOUNDARIES
7 Environmental Product Declaration DuPont de Nemours (Luxembourg) s.à r.l. – Tyvek® 2506B
lairetam
waR
ylppus tropsnarT
gnirutcafunaM
eht
morf
tropsnarT
etis
eht
ot
etag
ylbmessA esU
ecnanetniaM
riapeR
tnemecalpeR tnemhsibrufeR
ygrene
lanoitarepO esu
retaw
lanoitarepO esu
noitcurtsnoc-eD
noitilomed tropsnarT
gnissecorp
etsaW
lasopsiD -esueR -yrevoceR -gnilcyceR laitnetop
A1 A2 A3 A4 A5 B1 B2 B3 B4 B5 B6 B7 C1 C2 C3 C4 D
X X X X X ND ND MNR MNR MNR ND ND ND ND ND X X
RESULTS OF THE LCA - ENVIRONMENTAL IMPACT according to EN 15804+A2: 1 m2 DuPont™ Tyvek®
2506B
Core Indicator Unit A1-A3 A4 A5 C4 D
Global warming potential - total [kg CO2-Eq.] 5.69E-1 1.55E-2 1.85E-3 5.42E-1 -3.26E-1
Global warming potential - fossil fuels [kg CO2-Eq.] 5.70E-1 1.51E-2 1.50E-4 5.42E-1 -3.25E-1
Global warming potential - biogenic [kg CO2-Eq.] -1.55E-3 2.14E-4 1.70E-3 -3.21E-5 -1.22E-3
GWP from land use and land use change [kg CO2-Eq.] 4.81E-4 1.04E-4 4.91E-8 0.00E+0 -1.42E-4
Depletion potential of the stratospheric ozone layer [kg CFC11-Eq.] 1.33E-11 1.24E-17 2.39E-19 3.57E-10 -2.27E-15
Acidification potential, accumulated exceedance [mol H+-Eq.] 2.00E-3 1.63E-4 3.89E-7 7.14E-5 -3.35E-4
Eutrophication, fraction of nutrients reaching freshwater
[kg P-Eq.] 5.49E-6 3.93E-8 3.68E-9 1.30E-9 -2.67E-7
end compartment
Eutrophication, fraction of nutrients reaching marine end
[kg N-Eq.] 3.58E-4 6.00E-5 1.70E-7 1.22E-5 -1.06E-4
compartment
Eutrophication, accumulated exceedance [mol N-Eq.] 3.86E-3 6.61E-4 1.58E-6 2.85E-4 -1.15E-3
Formation potential of tropospheric ozone photochemical
[kg NMVOC-Eq.] 1.17E-3 1.34E-4 6.85E-7 3.57E-5 -3.04E-4
oxidants
Abiotic depletion potential for non-fossil resources [kg Sb-Eq.] 7.92E-8 1.16E-9 5.04E-12 7.62E-15 -3.93E-8
Abiotic depletion potential for fossil resources [MJ] 1.41E+1 2.05E-1 8.54E-4 1.02E-1 -5.58E+0
Water (user) deprivation potential, deprivation-weighted [m³ world-Eq
1.20E-1 1.84E-4 8.61E-5 4.76E-2 -1.51E-2
water consumption (WDP) deprived]
RESULTS OF THE LCA - INDICATORS TO DESCRIBE RESOURCE USE according to EN 15804+A2: 1 m2
DuPont™ Tyvek® 2506B
Indicator Unit A1-A3 A4 A5 C4 D
Renewable primary energy as energy carrier [MJ] 1.28E+0 1.31E-2 8.75E-5 2.64E-3 -7.81E-1
Renewable primary energy resources as material utilization [MJ] 1.12E-3 -2.43E-14 -1.22E-16 3.13E-6 1.77E-12
Total use of renewable primary energy resources [MJ] 1.28E+0 1.31E-2 8.75E-5 2.65E-3 -7.81E-1
Non-renewable primary energy as energy carrier [MJ] 1.41E+1 2.05E-1 8.54E-4 1.02E-1 -5.58E+0
Non-renewable primary energy as material utilization [MJ] 3.21E-4 6.68E-6 1.67E-8 3.01E-10 -1.23E-4
Total use of non-renewable primary energy resources [MJ] 1.41E+1 2.05E-1 8.54E-4 1.02E-1 -5.58E+0
Use of secondary material [kg] 3.82E-3 0.00E+0 0.00E+0 0.00E+0 0.00E+0
Use of renewable secondary fuels [MJ] 1.82E-6 0.00E+0 0.00E+0 0.00E+0 0.00E+0
Use of non-renewable secondary fuels [MJ] 1.97E-5 0.00E+0 0.00E+0 0.00E+0 0.00E+0
Use of net fresh water [m³] 6.45E-3 1.44E-5 2.05E-6 1.11E-3 -7.64E-4
RESULTS OF THE LCA – WASTE CATEGORIES AND OUTPUT FLOWS according to EN 15804+A2:
1 m2 DuPont™ Tyvek® 2506B
Indicator Unit A1-A3 A4 A5 C4 D
Hazardous waste disposed [kg] 3.70E-8 1.08E-11 1.54E-13 0.00E+0 -1.17E-9
Non-hazardous waste disposed [kg] 4.29E-3 3.35E-5 4.46E-4 0.00E+0 -2.06E-3
Radioactive waste disposed [kg] 1.91E-4 1.40E-6 1.79E-8 5.79E-6 -2.49E-4
Components for re-use [kg] 0.00 0.00 0.00 0.00 0.00
Materials for recycling [kg] 0.00 0.00 0.00 0.00 0.00
Materials for energy recovery [kg] 0.00 0.00 0.00 0.00 0.00
Exported electrical energy [MJ] 0.00E+0 0.00E+0 1.46E-3 8.86E-1 0.00E+0
Exported thermal energy [MJ] 0.00E+0 0.00E+0 2.08E-3 2.91E+0 0.00E+0
RESULTS OF THE LCA – additional impact categories according to EN 15804+A2-optional:
1 m2 DuPont™ Tyvek® 2506B
Indicator Unit A1-A3 A4 A5 C4 D
Potential incidence of disease due to PM emissions [Disease
ND ND ND ND ND
Incidence]
Potential Human exposure efficiency relative to U235 [kBq U235-
ND ND ND ND ND
Eq.]
Potential comparative toxic unit for ecosystems [CTUe] ND ND ND ND ND
Potential comparative toxic unit for humans - cancerogenic [CTUh] ND ND ND ND ND
Potential comparative toxic unit for humans - not cancerogenic [CTUh] ND ND ND ND ND
Potential soil quality index [-] ND ND ND ND ND
8 Environmental Product Declaration DuPont de Nemours (Luxembourg) s.à r.l. – Tyvek® 2506B
6. LCA: Interpretation
The following chart shows the relative contributions of
the different modules to the various LCA categories in
a dominance analysis.
For most of the impact categories, more than 70 % of
the impact is dominated by the functional layer (HDPE ADPE: Abiotic depletion potential for non-fossil
granulates and steam supply mainly) and lamination resources
(SBPP supply mainly) production steps; except for ADPF: Abiotic depletion potential for fossil resources
ODP which is dominated by the incineration of the FEP: Eutrophication, fraction of nutrients reaching
product after its use. freshwater end compartment
The production phase represents 53 % of the GWP, GWP: Global Warming Potential
which is also highly influenced by the final production HDPE: High-Density Polyethylene
incineration (46 % of the generated impact), due to Lam.: Lamination process
carbon dioxide emissions. LCA: Life Cycle Assessment
This outcome is coherent with the results for the MEP: Eutrophication, fraction of nutrients reaching
monolayers and with the fact that a large amount of marine end compartment
SBPP is used for the laminates. The avoided energy Mono: Monolayer production
production thanks to waste incineration leads to Nat. gas: Natural gas
significant benefits, which are mostly around 20 % of ODP: Depletion potential of the stratospheric ozone
the impact results (a bit higher than for monolayer layer
thanks to higher product weight). The module „EU-28: POCP: Formation potential of tropospheric ozone
Waste incineration of plastics (PE, PP, PS, PB)“ used photochemical oxidant
for the end-of-life of laminate dominates the ODP SBPP: Spunbond Polypropylene
score. TEP: Eutrophication, accumulated exceedance
WDP: Water (user) deprivation potential, deprivation-
Glossary: weighted water consumption
7. Requisite evidence
No requisite evidence is required for DuPont™ Tyvek®
2506B laminate membranes.
9 Environmental Product Declaration DuPont de Nemours (Luxembourg) s.à r.l. – Tyvek® 2506B
8. References
EN 12310-1
EN 12310-1:1999, Flexible sheets for waterproofing - ISO 14025
Part 1: Bitumen sheets for roof waterproofing; DIN EN ISO 14025:2011-10, Environmental labels and
determination of resistance to tearing (nail shank) declarations — Type III environmental declarations —
Principles and procedures.
EN 12311-1
EN 12311-1:1999, Flexible sheets for waterproofing - PCR, Part A
Part 1: Bitumen sheets for roof waterproofing; PCR 2021, Part A - PCR Guidance-Calculation Rules
Determination of tensile properties for the Life Cycle Assessment and Requirements on
the Project Report according to EN 15804+A2:2019
EN 1297 (version 1.1.1, 2021)
EN 1297:2004, Flexible sheets for waterproofing -
Bitumen, plastic and rubber sheets for roof PCR, Part B
waterproofing - Method of artificial ageing by long term PCR 2017, Part B - PCR Guidance-Texts for Building-
exposure to the combination of UV radiation, elevated Related Products and Services: Requirements on the
temperature and water EPD for False ceiling and underlay sheeting (version
1.6, 2017)
EN 13501-1
EN 13501-1:2007+A1:2010, Fire classification of IBU 2016
construction products and building elements - Part 1: Institut Bauen und Umwelt e.V.: General Programme
Classification using data from reaction to fire tests Instructions for the Preparation of EPDs at the Institut
Bauen und Umwelt e.V. Version 1., Berlin: Institut
EN 13859-1 Bauen und Umwelt e.V., 2016. www.ibu-epd.com
EN 13859-1:2010, Flexible sheets for waterproofing -
Definitions and characteristics of underlays - Part 1: BNB Nutzungsdauerliste
Underlays for discontinuous roofing BNB Nutzungsdauerliste: 2017. Nutzungsdaueren von
Bauteilen published by Informationsportal Nachhaltiges
EN 13859-2 Bauen des Bundesministeriums des Inneren für Bau
EN 13859-2:2010, Flexible sheets for waterproofing - und Heimat.
Definitions and characteristics of underlays - Part 2:
Underlays for walls European Waste Code
European Waste Code:2000. European List of Waste
EN 15804 European Waste Codes: (Commission decision
EN 15804:2019+A2, Sustainability of construction 2014/955/EU)
works — Environmental Product Declarations — Core
rules for the product category of construction products. Eurostat
Eurostat:2021, Data browser, Packaging waste by
EN 1848-2 waste management operations; Recycling rate of
EN 1848-2:2001, Flexible sheets for waterproofing - packaging waste by type of packaging
Determination of length, width, straightness and
flatness - Part 2: Plastic and rubber sheets for roof GaBi 10.5.0.78
waterproofing GaBi 10.5.0.78:2021. Life Cycle Engineering software
and database. Sphera Solutions GmbH, 2021.
EN 1849-2
EN 1849-2:2019, Flexible sheets for waterproofing - Regulation (EU) No. 305/2011
Determination of thickness and mass per unit area - Regulation (EU) No. 305/2011 of the European
Part 2: Plastic and rubber sheets Parliament and of the Council of 9 March 2011 laying
down harmonised conditions for the marketing of
EN 1928 construction products and repealing Council Directive
EN 1928:2000, Flexible sheets for waterproofing - 89/106/EEC
Bitumen, plastic and rubber sheets for roof
waterproofing - Determination of watertightness DuPont™, the DuPont Oval Logo, and
all trademarks and service marks denoted with ™,
EN ISO 12572 SM or ® are owned by affiliates of DuPont de
EN ISO 12572:2017, Hygrothermal performance of Nemours, Inc. unless otherwise noted.
building materials and products -- Determination of
water vapour transmission properties
EN ISO 14001
EN ISO 14001:2015, Environmental management
systems - Requirements with guidance for use (ISO
14001:2015)
10 Environmental Product Declaration DuPont de Nemours (Luxembourg) s.à r.l. – Tyvek® 2506B
Publisher
Institut Bauen und Umwelt e.V. Tel +49 (0)30 3087748- 0
Panoramastr. 1 Fax +49 (0)30 3087748- 29
10178 Berlin Mail info@ibu-epd.com
Germany Web www.ibu-epd.com
Programme holder
Institut Bauen und Umwelt e.V. Tel +49 (0)30 - 3087748- 0
Panoramastr 1 Fax +49 (0)30 – 3087748 - 29
10178 Berlin Mail info@ibu-epd.com
Germany Web www.ibu-epd.com
Author of the Life Cycle
Assessment Tel 00352-275888-1
Luxembourg Institute of Science Fax 00352-275888-555
and Technology (LIST) Mail info@list.lu
Avenue des Hauts-Fourneaux 5 Web www.list.lu
4362 Esch/Alzette
Luxembourg
Owner of the Declaration
DuPont de Nemours (Luxembourg) Tel +352 3666 5210
s.à r.l. Fax +352 3666 0000
Rue Général Patton 1 Mail tyvek.info@dupont.com
2984 Contern Web www.dupont.com
Luxembourg
