ENVIRONMENTAL PRODUCT DECLARATION
as per ISO 14025 and EN 15804+A2
Owner of the Declaration Würth Group / Adolf Würth GmbH & Co. KG
Publisher Institut Bauen und Umwelt e.V. (IBU)
Programme holder Institut Bauen und Umwelt e.V. (IBU)
Declaration number EPD-AWU-20230570-CBA1-EN
Issue date 21.03.2024
Valid to 20.03.2029
Steel Screws
Adolf Würth GmbH & Co. KG
www.ibu-epd.com | https://epd-online.com
General Information
Adolf Würth GmbH & Co. KG Steel Screws
Programme holder Owner of the declaration
IBU – Institut Bauen und Umwelt e.V. Würth Group / Adolf Würth GmbH & Co. KG
Hegelplatz 1 Reinhold-Würth Str. 12-17
10117 Berlin 74653 Künzelsau
Germany Germany
Declaration number Declared product / declared unit
EPD-AWU-20230570-CBA1-EN 1 kg weighted average of dowel-type fasteners with thread.
This declaration is based on the product category rules: Scope:
Screws, 01.06.2023 This EPD relates to timber screws, chipboard screws, drilling and tapping
(PCR checked and approved by the SVR) screws, screws for plastics, metric screws and dowel-type fasteners with
thread made of steel or stainless steel. Depending on the type of screw,
these products are generally used for fastening two or more components
Issue date made of wood, steel or plastic.
21.03.2024
The declared environmental data related to 1 kg of steel are based on a
weighted average of steel screws in a Würth manufacturing plant, SWG
Schraubenwerk Gaisbach GmbH and internationalized with generic data.
Valid to
The holder of the declaration shall be liable for the underlying information
20.03.2029 and supporting documents; any liability of IBU (Institut Bauen und Umwelt
e. V.) with regard to manufacturer information, life cycle assessment data
and supporting documents is hereby excluded. The EPD (Environmental
Product Declaration) was created in accordance with EN 15804 + A2:
2022-03. In the following, the standard is referred to in simplified form as
EN 15804.
The owner of the declaration shall be liable for the underlying information
and evidence; the IBU shall not be liable with respect to manufacturer
information, life cycle assessment data and evidences.
The EPD was created according to the specifications of EN 15804+A2. In
the following, the standard will be simplified as EN 15804.
Dipl.-Ing. Hans Peters
(Chairman of Institut Bauen und Umwelt e.V.)
Verification
The standard EN 15804 serves as the core PCR
Independent verification of the declaration and data according to ISO
14025:2011
internally X externally
Florian Pronold Dr.-Ing. Nikolay Minkov,
(Managing Director Institut Bauen und Umwelt e.V.) (Independent verifier)
1 Environmental Product Declaration - Adolf Würth GmbH & Co. KG - Steel Screws
Product
Depending on the type of screw, these products are generally
Product description/Product definition used for fastening components made of wood, steel or plastic.
Dowel-type fasteners with thread, e.g. screws made of steel, Possible application examples include timber construction, steel
are fasteners that can predominantly be used for fastening two construction, indoor/outdoor use, furniture applications or
or more components. The materials to be fastened or screw-in window construction. Examples of Würth product groups are
surfaces can be made of wood, wood materials, plastic, ASSY, Pias and Piasta screws.
aluminium, steel, stainless steel or other metals.
Technical Data
Pin-shaped connectors, such as screws, are generally Structural data for the respective dowel-type fasteners with
manufactured from a wire (steel) and provided with a head on thread are provided in the corresponding approvals and
one component side to be tightened. Depending on the technical drawings, as shown below in an excerpt from ETA
application, it can have different shapes, e.g. countersunk 11/0190 (ASSY) for wood screws.
head, round head, hexagon head or washer head. For
Constructional data
anchoring the pin-shaped connectors, a thread is formed on the
Data based on ASSY plus VG:
opposite side. The thread shape (e.g. wood thread or metric
thread) is matched to the screw-in surface and can be designed Name Value Unit
differently in terms of thread height, thread angle or thread Screw diameter 8 mm
pitch. The point design of the dowel-type fasteners with thread Usage category as per ETA 11/0190 -
is matched to the application, e.g. wooden tip, drill tip or blunt
Characteristic tension resistance 20 kN
shape. For protection against corrosion or e.g. for setting a
Screw length (+1.0/-0.5) 450 - 480 mm
sliding friction, the pin-shaped connectors can be provided with
different coatings, for example, zinc or anti-skid coating. Material carbone steel
Product according to CPR with hEN:
Depending on the application, the additional use of suitable
• Performance values of the product in accordance with
steel or stainless steel seals as well as EPDM seals (ethylene-
the declaration of performance in relation to its essential
propylene-diene rubber), washers or nuts is provided.
characteristics according to applicable hEN such as EN
Depending on the application, the dowel-type fasteners with
15048-1:2016 and EN 14399-1:2015.
thread can be subject to legal national or European
requirements such as the Construction Products Regulation.
Product according to CPR with ETA:
For example, the following documentation possibilities may be
available: • Performance values of the product according to the
declaration of performance with respect to its essential
Product according to CPR with hEN: characteristics in accordance with applicable ETA.
Regulation (EU) No 305/2011 (CPR) shall apply to the placing
of the product on the market in the European Union/European Product that is not subject to EU harmonization legislation:
Free Trade Association (EU/EFTA) states (with the exception of • Performance values of the product in relation to its
Switzerland). The product requires a declaration of characteristics according to the applicable technical
performance taking into account the respective EN. regulation (no CE marking).
All approvals can be downloaded from the Würth Online Shop
The CE marking shall be applied to the product in compliance homepage under the Documents tab for the respective
with the proof of its conformity with the following harmonized products.
standards based on the mentioned harmonization legislation:
• EN 14592:2008-04; timber structures - dowel-type
Base materials/Ancillary materials
fasteners
The use shall be subject to the respective national provisions. Dowel-type fasteners with thread are made of steel. As
explained in the product description , depending on the type of
Product according to CPR with ETA: application and material, the fasteners are provided with, for
Regulation (EU) No 305/2011 (CPR) shall apply to the placing example, galvanic and/or mechanical galvanizing and, if
of the product on the market in the European Union/European appropriate, with anti-friction coating. Depending on the
Free Trade Association (EU/EFTA) states (with the exception of application, the fasteners are also equipped with a
Switzerland). The product needs a declaration of performance corresponding sealing washer made of steel, stainless steel or
taking into account the respective ETA such as ETA-10/0184, aluminum and EPDM sealing rubber.
ETA-13/0210 or ETA-11/0190 and CE marking.
Steel
The use shall be subject to the respective national provisions. Steel is an iron-carbon alloy, which is also referred to as a
metallic alloy. It contains less than 2.06 % (by mass) carbon.
Product that is not subject to EU harmonization legislation: DIN EN 10020 also defines steels as materials in which the iron
The national regulations of the place of use apply to the use of content is higher than that of any other element and the carbon
the product. In Germany, for example, the building codes of the content is generally below 2 % by weight. Steel is a chemical
respective countries and the technical building regulations alloy of iron and iron carbide.
based on these codes apply.
Compared to cast iron, which contains a higher carbon content
and graphite as carbon form, steel can be processed by
Application technical forming.
Timber screws, chipboard screws, drilling and tapping screws,
plastic screws and dowel-type fasteners with thread made of EPDM
steel are used when fastening two or more components. EPDM is an abbreviation for ethylene-propylene diene
2 Environmental Product Declaration - Adolf Würth GmbH & Co. KG - Steel Screws
(monomer) rubber and is a terpolymer elastomer (rubber). It lubricants. Depending on the application, these include
thus belongs to the group of synthetic rubbers. In the context of kerosenes, polymers and waxes. A lubricious coating is applied
the rubber classification, seals made of this sealing material are to the screw by means of an immersion bath or drum coating. It
therefore assigned to the group of non-polar saturated rubbers. lies on the screw as a dry transparent film. Some lubricating
This material is a high-quality rubber-elastic synthetic elastomer coatings contain small amounts of alcohol. Type 6 work
of ethylene, propylene and dienes of high-molecular weight. clothing, safety goggles, face protection and chemical-resistant
The saturated basic molecular base structure of EPDM offers gloves are worn as safety measures to protect human contact
properties such as high weathering resistance, ozone during coating. An annual safety briefing is carried out and
resistance and high heat resistance. extraction systems are used.
Electrogalvanizing Reference service life
Galvanization (also electroplating technology) is a surface and Given the wide range of applications, no specific information on
coating technology process for the electrochemical separation the recommended useful life is provided. The actual service life
of metals on metallic or metallized surfaces using an electrolyte of screws generally depends on their intended use, installation
and direct current. Functional electroplating protects against environment and proper installation. External influences can
corrosion and wear, catalyzes, improves conductivity, and have a significant impact on the useful life. According to the
reduces frictional forces. The ductility and formability of European Technical Approval, the average useful life of screws
workpieces can also be influenced by electroplating. is > 25 years. The indication of the useful life cannot be
understood as a guarantee by the manufacturer. It must be
Anti-friction coating ensured that the use of the dowel-type fasteners with thread
Aqueous suspensions, emulsions and dispersions are used as complies with the applicable technical regulations.
LCA: Calculation rules
but is not recommended, as the slide coating can be destroyed
Declared Unit by the initial screw-in process and the function of the fastener
1 kg average self-tapping screws made of steel: can no longer be guaranteed after repeated use.
Declared unit and mass reference · C2 transport to waste processing; 50 km with truck Transport
distance can be adjusted at building level if necessary (e.g., for
Name Value Unit
100 km actual transport distance: multiply LCA values by factor
Declared unit 1 kg
2)
Gross density 7900 kg/m3 · C3 waste processing for recycling of steel.
· C4 no components of the product are landfilled.
The exact weight of the screw is provided digitally.
System boundary
Type of the EPD: cradle-to-gate - with options, modules C1-C4 Benefits and loads beyond the System Boundary (D): Module D
and module D (A1-A3 + C + D and additional modules: A4, A5). includes:
Material recovery potentials from metal recycling and energy
Production Stage (A1-A3): The Product stage includes: recovery potentials from the
· A1 Raw material supply and processing (mainly steel), thermal recovery of Packaging.
· A2 Transport of raw materials to the manufacturer,
Geographic Representativeness
· A3 Production of Stainless steel screws (incl. energy
Land or region, in which the declared product system is
provision, treatment of production waste, production of
manufactured, used or handled at the end of the product´s
packaging materials).
lifespan: Global
Construction stage (A4-A5): The construction process stage
includes: Comparability
· A4 transport to the construction site 100 km by truck,
Basically, a comparison or an evaluation of EPD data is only
· A5 Disposal of the packaging and installation of the Stainless
possible if all the data sets to be compared were created
steel screw.
according to EN 15804 and the building context, respectively
the product-specific characteristics of performance, are taken
into account. The underlying database is LCA FE (GaBi) 2023,
End-of-life stage (C1-C4): The end-of-life stage includes:
version 2023.1
· C1 machine-assisted de- construction (Hand-screwdriver;
battery operated); Direct reuse would theoretically be possible,
LCA: Scenarios and additional technical information
Characteristic product properties of biogenic carbon
Information on describing the biogenic carbon content at
factory gate
Note: 1 kg of biogenic carbon is equivalent to 44/12 kg of CO2 Transport from the gate to the site (A4)
Name ValueUnit Name Value Unit
kg Litres of fuel (per kg transported goods) 0.0018 l/100km
Biogenic carbon content in product -
C Transport distance 100 km
Biogenic carbon content in accompanying kg Capacity utilisation (including empty runs) 61 %
0.023
packaging C
Mass for transportation 1 kg
3 Environmental Product Declaration - Adolf Würth GmbH & Co. KG - Steel Screws
Assembly (A5) Reuse, recovery and/or recycling potentials (D), relevant
Name Value Unit scenario information
Electricity consumption 0.0281kWh Name Value Unit
Material loss - kg collection rate 100 %
Output substances following waste treatment on The results of the scenario (100%) can be scaled on building
0.053 kg
site (Packaging) level according to the applied collection rate.
End of life (C1-C4)
Name Value Unit
Electricity consumption for dismantling 0.0281 kWh
Collected separately waste type waste type 1 kg
Collected as mixed construction waste - kg
Reuse - kg
Recycling 1 kg
Energy recovery - kg
4 Environmental Product Declaration - Adolf Würth GmbH & Co. KG - Steel Screws
LCA: Results
DESCRIPTION OF THE SYSTEM BOUNDARY (X = INCLUDED IN LCA; MND = MODULE OR INDICATOR NOT DECLARED; MNR
= MODULE NOT RELEVANT)
Benefits and
Construction loads beyond
Product stage Use stage End of life stage
process stage the system
boundaries
la ire ta m w a Ry lp p u s tro p s n a rT g n iru tc a fu n a M e h t m o rf tro p s n a rTe tis e h t o t e ta g y lb m e s s A e s U e c n a n e tn ia M ria p e R tn e m e c a lp e R tn e m h s ib ru fe R y g re n e la n o ita re p Oe s u re ta w la n o ita re p Oe s u n o itc u rts n o c -e Dn o itilo m e d tro p s n a rT g n is s e c o rp e ts a W la s o p s iD -e s u e R-y re v o c e R-g n ilc y c e Rla itn e to p
A1 A2 A3 A4 A5 B1 B2 B3 B4 B5 B6 B7 C1 C2 C3 C4 D
X X X X X MND MND MNR MNR MNR MND MND X X X X X
RESULTS OF THE LCA - ENVIRONMENTAL IMPACT according to EN 15804+A2: 1 kg Steel fasteners with thread
Parameter Unit A1-A3 A4 A5 C1 C2 C3 C4 D
GWP-total kg CO 2 eq 3.25E+00 6.69E-03 1.24E-01 4.26E-02 4.34E-03 0 0 -1.64E+00
GWP-fossil kg CO 2 eq 3.32E+00 6.61E-03 4.5E-02 4.26E-02 4.29E-03 0 0 -1.65E+00
GWP-biogenic kg CO 2 eq -7.54E-02 1.95E-05 7.86E-02 2.12E-05 1.27E-05 0 0 3.04E-03
GWP-luluc kg CO 2 eq 2.69E-03 6.13E-05 4.3E-06 3.9E-06 3.98E-05 0 0 -6.74E-04
ODP kg CFC11 eq 3.17E-12 8.61E-16 4.28E-13 4.19E-13 5.59E-16 0 0 4.58E-12
AP mol H+ eq 1E+00 9.86E-06 8.45E-05 6.49E-05 6.4E-06 0 0 -3.68E-03
EP-freshwater kg P eq 3.97E-06 2.42E-08 4.49E-08 4.21E-08 1.57E-08 0 0 -1.57E-07
EP-marine kg N eq 1.06E-01 3.6E-06 2.54E-05 1.83E-05 2.34E-06 0 0 -8.85E-04
EP-terrestrial mol N eq 1.16E+00 4.25E-05 2.82E-04 1.93E-04 2.76E-05 0 0 -9.58E-03
kg NMVOC
POCP 3.29E-01 8.66E-06 6.95E-05 5.06E-05 5.62E-06 0 0 -2.94E-03
eq
ADPE kg Sb eq 2.13E-05 4.36E-10 2.14E-09 2.06E-09 2.83E-10 0 0 -1.85E-08
ADPF MJ 3.52E+01 9.01E-02 9.59E-01 9.36E-01 5.85E-02 0 0 -1.24E+01
m3 world eq
WDP 1.38E-01 7.99E-05 1.24E-02 3.58E-03 5.19E-05 0 0 -2.52E-02
deprived
GWP = Global warming potential; ODP = Depletion potential of the stratospheric ozone layer; AP = Acidification potential of land and water; EP =
Eutrophication potential; POCP = Formation potential of tropospheric ozone photochemical oxidants; ADPE = Abiotic depletion potential for non-fossil
resources; ADPF = Abiotic depletion potential for fossil resources; WDP = Water (user) deprivation potential)
RESULTS OF THE LCA - INDICATORS TO DESCRIBE RESOURCE USE according to EN 15804+A2: 1 kg Steel fasteners with
thread
Parameter Unit A1-A3 A4 A5 C1 C2 C3 C4 D
PERE MJ 3.15E+00 6.56E-03 1.03E+00 1.28E-01 4.26E-03 0 0 1.87E+00
PERM MJ 9E-01 0 -9E-01 0 0 0 0 0
PERT MJ 4.05E+00 6.56E-03 1.34E-01 1.28E-01 4.26E-03 0 0 1.87E+00
PENRE MJ 3.53E+01 9.05E-02 9.73E-01 9.36E-01 5.87E-02 0 0 -1.26E+01
PENRM MJ 1.38E-02 0 -1.38E-02 0 0 0 0 0
PENRT MJ 3.53E+01 9.05E-02 9.59E-01 9.36E-01 5.87E-02 0 0 -1.26E+01
SM kg 2.03E-01 0 0 0 0 0 0 8.08E-01
RSF MJ 0 0 0 0 0 0 0 0
NRSF MJ 0 0 0 0 0 0 0 0
FW m3 3.76E-03 7.18E-06 4.23E-04 2.15E-04 4.66E-06 0 0 -1.13E-03
PERE = Use of renewable primary energy excluding renewable primary energy resources used as raw materials; PERM = Use of renewable primary
energy resources used as raw materials; PERT = Total use of renewable primary energy resources; PENRE = Use of non-renewable primary energy
excluding non-renewable primary energy resources used as raw materials; PENRM = Use of non-renewable primary energy resources used as raw
materials; PENRT = Total use of non-renewable primary energy resources; SM = Use of secondary material; RSF = Use of renewable secondary fuels;
NRSF = Use of non-renewable secondary fuels; FW = Use of net fresh water
RESULTS OF THE LCA – WASTE CATEGORIES AND OUTPUT FLOWS according to EN 15804+A2:
1 kg Steel fasteners with thread
Parameter Unit A1-A3 A4 A5 C1 C2 C3 C4 D
HWD kg 1.23E-08 2.8E-13 5.5E-11 5.43E-11 1.82E-13 0 0 -5.33E-11
NHWD kg 3.76E-02 1.38E-05 2.5E-03 2.06E-04 8.95E-06 0 0 -2.43E-02
RWD kg 4.98E-04 1.69E-07 1.47E-04 1.46E-04 1.1E-07 0 0 1.8E-04
CRU kg 0 0 0 0 0 0 0 0
MFR kg 1.01E-02 0 0 0 0 1E+00 0 0
MER kg 0 0 0 0 0 0 0 0
EEE MJ 0 0 1.09E-01 0 0 0 0 0
5 Environmental Product Declaration - Adolf Würth GmbH & Co. KG - Steel Screws
EET MJ 0 0 1.97E-01 0 0 0 0 0
HWD = Hazardous waste disposed; NHWD = Non-hazardous waste disposed; RWD = Radioactive waste disposed; CRU = Components for re-use;
MFR = Materials for recycling; MER = Materials for energy recovery; EEE = Exported electrical energy; EET = Exported thermal energy
RESULTS OF THE LCA – additional impact categories according to EN 15804+A2-optional:
1 kg Steel fasteners with thread
Parameter Unit A1-A3 A4 A5 C1 C2 C3 C4 D
Disease
PM 5.43E-06 8.16E-11 6.95E-10 5.87E-10 5.3E-11 0 0 -5.36E-08
incidence
IR kBq U235 eq 4.53E-02 2.52E-05 2.21E-02 2.19E-02 1.64E-05 0 0 1.81E-02
ETP-fw CTUe 6.61E+00 6.4E-02 2.79E-01 2.68E-01 4.16E-02 0 0 -2.17E+00
HTP-c CTUh 4.09E-09 1.31E-12 5.43E-12 4.84E-12 8.5E-13 0 0 -2.5E-09
HTP-nc CTUh 1.57E-07 6.98E-11 2.72E-10 2.48E-10 4.54E-11 0 0 -9.82E-09
SQP SQP 1.38E+01 3.77E-02 1.33E-01 1.27E-01 2.45E-02 0 0 1.05E+00
PM = Potential incidence of disease due to PM emissions; IR = Potential Human exposure efficiency relative to U235; ETP-fw = Potential comparative
Toxic Unit for ecosystems; HTP-c = Potential comparative Toxic Unit for humans (cancerogenic); HTP-nc = Potential comparative Toxic Unit for humans
(not cancerogenic); SQP = Potential soil quality index
Disclaimer 1 – for the indicator “Potential Human exposure efficiency relative to U235”. This impact category deals mainly with the
eventual impact of low-dose ionizing radiation on human health of the nuclear fuel cycle. It does not consider effects due to possible
nuclear accidents, occupational exposure or radioactive waste disposal in underground facilities. Potential ionizing radiation from the
soil, radon and from some construction materials is also not measured by this indicator.
Disclaimer 2 – for the indicators “abiotic depletion potential for non-fossil resources”, “abiotic depletion potential for fossil resources”,
“water (user) deprivation potential, deprivation-weighted water consumption”, “potential comparative toxic unit for ecosystems”,
“potential comparative toxic unit for humans – cancerogenic”, “Potential comparative toxic unit for humans - not cancerogenic”,
“potential soil quality index”. The results of this environmental impact indicator shall be used with care as the uncertainties on these
results are high as there is limited experience with the indicator.
References
Standards Leinfelden Echterdingen
EN 15804 GaBi documentation
EN 15804:2012+A1 2013, Sustainability of construction works GaBi life cycle inventory data documentation
— Environmental Product Declarations — Core rules for the (http://www.gabi-software.com/international/databases/gabi-
product category of construction products. data-search/)
EN 15804 IBU 2021
EN 15804:2012+A2:2019+AC:2021, Sustainability of Institut Bauen und Umwelt e.V.: General Programme
construction works — Environmental Product Declarations — Instructions
Core rules for the product category of construction products. for the Preparation of EPDs at the Institut Bauen und Umwelt
e.V., version 2.0., Berlin: Institut Bauen und Umwelt e.V., 2021,
EN 14592 http://www.ibu-epd.com
EN 14592:2008-04, Timberstructures– Dowel-typefasteners–
Requirements PCR Part A
Calculation Rules for the Life Cycle Assessment and
ISO 14025 Requirements on the Project Report,Berlin: Institut Bauen und
EN ISO 14025:2011, Environmental labels and declarations — Umwelt e.V., www.ibu-epd.com, Version 1.3, 2021
Type III environmental declarations — Principles and
procedures. PCR Part B
Requirements on the EPD for Screws ,
DIN EN 10020 version 8, Institut Bauen und Umwelt e.V., www.bau-
DIN EN 10020:2000, Definition and classification of grades of umwelt.com, 2023
steel
ETA-11/0190 (ASSY)
Literature
ETA-10/0184
GaBi software
Sphera Solutions GmbH ETA-13/0210
GaBi Software System and Database for Life Cycle
Engineering Regulation (EU) No 305/2011 (CPR)
CUP Version: 2023.1
University of Stuttgart
6 Environmental Product Declaration - Adolf Würth GmbH & Co. KG - Steel Screws
Publisher
Institut Bauen und Umwelt e.V. +49 (0)30 3087748- 0
Hegelplatz 1 info@ibu-epd.com
10117 Berlin www.ibu-epd.com
Germany
Programme holder
Institut Bauen und Umwelt e.V. +49 (0)30 3087748- 0
Hegelplatz 1 info@ibu-epd.com
10117 Berlin www.ibu-epd.com
Germany
Author of the Life Cycle Assessment
Sphera Solutions GmbH +49 711 341817-0
Hauptstraße 111- 113 info@sphera.com
70771 Leinfelden-Echterdingen www.sphera.com
Germany
Owner of the Declaration
Würth Group / Adolf Würth GmbH & Co. KG +49 7940 15-0
Reinhold-Würth Str. 12-17 info@wuerth.com
74653 Künzelsau www.wuerth.com
Germany
Adolf Würth GmbH & Co. KG +49 7940/15-0
Reinhold-Würth-Str. 12-17 info@wuerth.com
74653 Künzelsau www.wuerth.de
Germany
Würth Industrie Service GmbH & Co. KG +49 7931 91-0
Industriepark Würth, Drillberg - info@wuerth-industrie.com
97980 Bad Mergentheim www.wuerth-industrie.com
Germany
7 Environmental Product Declaration - Adolf Würth GmbH & Co. KG - Steel Screws
