ENVIRONMENTAL PRODUCT DECLARATION
as per ISO 14025 and EN 15804+A2
Owner of the Declaration dormakaba International Holding GmbH
Publisher Institut Bauen und Umwelt e.V. (IBU)
Programme holder Institut Bauen und Umwelt e.V. (IBU)
Declaration number EPD-DOR-20220158-CBA1-EN
Issue date 29.11.2022
Valid to 28.11.2027
DL 200/300
dormakaba
www.ibu-epd.com | https://epd-online.com
General Information
dormakaba DL 200/300
Programme holder Owner of the declaration
IBU – Institut Bauen und Umwelt e.V. dormakaba International Holding GmbH
Hegelplatz 1 DORMA Platz 1
10117 Berlin 58256 Ennepetal
Germany Germany
Declaration number Declared product / declared unit
EPD-DOR-20220158-CBA1-EN 1 Mortise Lock (1 piece) of the DL 300 Series, consisting of the following
items:
- one (1) mortise lock DL 300
- one (1) closed case
- one (1) forend
- packaging
This declaration is based on the product category rules: Scope:
Building Hardware products, 01.08.2021 This declaration is a specific product declaration for the Mortise Lock
(PCR checked and approved by the SVR) Series DL 300 manufactured by dormakaba production facility Wah Yuet.
The production site is located in Guangdong Province, China. This
Environmental Product Declaration is also representative for the DL 200
Issue date Mortise Lock Series. The underlying life cycle assessment is based on the
entire life cycle of this specific mortise lock series. Data represents the
29.11.2022
year 2021.
The owner of the declaration shall be liable for the underlying information
and evidence; the IBU shall not be liable with respect to manufacturer
Valid to
information, life cycle assessment data and evidences.
28.11.2027
The EPD was created according to the specifications of EN 15804+A2. In
the following, the standard will be simplified as EN 15804.
Verification
The standard EN 15804 serves as the core PCR
Independent verification of the declaration and data according to ISO
14025:2011
internally X externally
Dipl.-Ing. Hans Peters
(Chairman of Institut Bauen und Umwelt e.V.)
Florian Pronold Dr.-Ing. Wolfram Trinius,
(Managing Director Institut Bauen und Umwelt e.V.) (Independent verifier)
1 Environmental Product Declaration - dormakaba - DL 200/300
Product
Performance data of the product with respect to its
Product description/Product definition characteristics in accordance with the relevant technical
dormakaba mortise lock series DL 200/300 for timber and steel provision which can be applied are mentioned above.
doors. DL 200/300 is a complementary Euro-Size lockset
series. A range of mechanically operated locks for doors in Delivery status:
buildings. A complete range of high-quality products and One (1) serial standard DL 300 Mortise Lock includes
functional reliability. With the use of high-grade materials,
precise production techniques and a comprehensive quality one (1) DL 300 lock, one (1) closed case and one forend.
management system, all dormakaba locks meet demanding Including packaging the DL 300 Mortise Lock will be supplied
technical specifications. with a weight of 1,35 kg.
Locks are supplied complete with fixing screws, strike plate and
dust box. Base materials/Ancillary materials
The material composition of the product is the following:
For the use and application of the product the respective Name Value Unit
national provisions at the place of use apply. dormakaba locks
Stainless steel 23,0 %
are subject to strict quality requirements and are tested and
Steel 57,0 %
certified according to:
Paper 0,7 %
• EN 12209:2003
Plastic 19,3 %
• DIN 18251:2020-04
For applications with increased security requirements the locks These figures are also representative for the DL 200 Mortise
are tested and certified in accordance with national and Lock system.
international standards.
The DL 200/300 Mortise Lock system contains articles which
Application
contain substances
dormakaba locks can be used universally on standard doors by listed in the Candidate List of REACH
changing the latch handing, without using a tool. Moreover, Regulation 1907/2006/EC (date: 10.06.2022)
they offer precision by simple, compatible assembling in exceeding 0.1 percentage by mass: no
standard door cuts. As well as for applications with increased
security requirements. dormakaba locks are as well fire-tested The candidate list can be found on the ECHA website address:
and Certifire-approved. https://echa.europe.eu/de/home.
Technical Data
The DL 200/300 Mortise Lock Series fullfils following technical Reference service life
properties: dormakaba DL 200/300 Mortise Lock Series are certified
according to EN 12209 up to 200.000 cycles of use. Under
normal conditions and depending on cycle frequency, door
weight and environmental conditions a duration of 15 years can
be secured.
LCA: Calculation rules
Production - Module A1-A3
Declared Unit The product stage includes:
The declared unit is 1 piece of the product: DL 300 Mortise — A1, raw material extraction, processing and mechanical
Lock Series. treatments, processing of secondary material input (e.g.
Declared unit recycling processes), — A2, transport to the manufacturer, —
A3, manufacturing and assembly including provision of all
Name Value Unit
materials, products and energy, as well as waste processing up
Declared unit 1 piece/product
to the end-of waste state.
Mass of declared Product 1.35 kg Construction stage - Modules A4-A5
The construction process stage includes:
System boundary — A4, transport to the building site; — A5, installation into the
The type of EPD is according to EN 15804: "cradle to gate with building; including provision of all materials, products and
options, modules C1–C4, and module D". energy, as well as waste processing up to the end-of waste
The following modules are declared: A1-A3, C1-C4, D and state or disposal of final residues during the construction
additional modules: A4 + A5 process stage.
2 Environmental Product Declaration - dormakaba - DL 200/300
End-of-life stage– Modules C1-C4 and D
The end-of-life stage includes: Geographic Representativeness
— C1, de-construction, demolition: Land or region, in which the declared product system is
— C2, transport to waste processing; — C3, waste processing manufactured, used or handled at the end of the product´s
for reuse, recovery and/or recycling; — C4, disposal; including lifespan: China
provision and all transport, provision of all materials, products
and related energy and water use.
Comparability
Module D (Benefits and loads beyond the system boundary)
Basically, a comparison or an evaluation of EPD data is only
includes:
possible if all the data sets to be compared were created
— D, recycling potentials, expressed as net impacts and
according to EN 15804 and the building context, respectively
benefits.
the product-specific characteristics of performance, are taken
into account. Background database: GaBi, SP40.
LCA: Scenarios and additional technical information
Installation into the building (A5)
Characteristic product properties of biogenic carbon
Name Value Unit
Information on describing the biogenic Carbon Content at
Output substances following waste treatment on
factory gate 0.25575 kg
site Waste packaging (paper)
Name ValueUnit
Biogenic carbon content in accompanying kg End of life (C1-C4)
0.09
packaging C C1: The product dismantling from the building is done manually
without environmental burden.
Note: 1 kg of biogenic carbon is equivalent to 44/12 kg of CO .
2
Name Value Unit
Collected separately waste type 1.1 kg
Additional technical information for the Recycling 1.09 kg
declared modules.
Energy recovery 0.0081 kg
Transport to the building site (A4)
The product is disassembled in a recycling process. Material
Name Value Unit recycling is then assumed for the metals. The plastic
Litres of fuel (per 1kg) 0.00276l/100km components are assumed to be incinerated with energy
Transport distance plane 6496 km recovery. Region for the End of Life is: Global.
Transport distance truck 168 km
Reuse, recovery and/or recycling potentials (D), relevant
Capacity utilisation (including empty runs)
55 % scenario information
average
Name Value Unit
The product is transported via plane and truck. The sales
markets have been considered to calculate the transport The collection rate is 100 %.
distances.
3 Environmental Product Declaration - dormakaba - DL 200/300
LCA: Results
DESCRIPTION OF THE SYSTEM BOUNDARY (X = INCLUDED IN LCA; MND = MODULE OR INDICATOR NOT DECLARED; MNR
= MODULE NOT RELEVANT)
Benefits and
Construction loads beyond
Product stage Use stage End of life stage
process stage the system
boundaries
la ire ta m w a Ry lp p u s tro p s n a rT g n iru tc a fu n a M e h t m o rf tro p s n a rTe tis e h t o t e ta g y lb m e s s A e s U e c n a n e tn ia M ria p e R tn e m e c a lp e R tn e m h s ib ru fe R y g re n e la n o ita re p Oe s u re ta w la n o ita re p Oe s u n o itc u rts n o c -e Dn o itilo m e d tro p s n a rT g n is s e c o rp e ts a W la s o p s iD -e s u e R-y re v o c e R-g n ilc y c e Rla itn e to p
A1 A2 A3 A4 A5 B1 B2 B3 B4 B5 B6 B7 C1 C2 C3 C4 D
X X X X X MND MND MNR MNR MNR MND MND MND X X MND X
RESULTS OF THE LCA - ENVIRONMENTAL IMPACT according to EN 15804+A2: DL200/300 Mortise Lock Series
Parameter Unit A1-A3 A4 A5 C2 C3 D
Global Warming Potential total (GWP-total) kg CO 2 eq 3.87E+00 3.29E-01 3.64E-01 5E-03 1.9E-02 -2.61E+00
Global Warming Potential fossil fuels (GWP-fossil) kg CO 2 eq 4.27E+00 3.28E-01 1.1E-02 5E-03 1.9E-02 -2.62E+00
Global Warming Potential biogenic (GWP-biogenic) kg CO 2 eq -4.07E-01 1E-03 3.54E-01 2.11E-04 4.44E-07 5E-03
Global Warming Potential luluc (GWP-luluc) kg CO 2 eq 4.93E-03 6.88E-06 6.05E-06 1.09E-07 1.08E-06 -3E-03
Depletion potential of the stratospheric ozone layer (ODP) kg CFC11 eq 2.84E-12 2.41E-17 6.61E-17 4.82E-19 9.61E-18 -1.67E-15
Acidification potential of land and water (AP) mol H+ eq 1.7E-02 1E-03 1.02E-04 4.57E-06 3.39E-06 -9E-03
Eutrophication potential aquatic freshwater (EP-freshwater) kg P eq 1.16E-05 5.4E-08 1.29E-08 9.78E-10 1.53E-09 -1.99E-06
Eutrophication potential aquatic marine (EP-marine) kg N eq 2.5E-03 5.76E-04 3.67E-05 1.46E-06 7.65E-07 -1E-03
Eutrophication potential terrestrial (EP-terrestrial) mol N eq 3.11E-02 6E-03 4.58E-04 1.62E-05 1.55E-05 -1.5E-02
Formation potential of tropospheric ozone photochemical oxidants kg NMVOC
8.02E-03 2E-03 9.74E-05 4.12E-06 2.12E-06 -5E-03
(POCP) eq
Abiotic depletion potential for non fossil resources (ADPE) kg Sb eq 1.1E-04 9.28E-09 1.04E-09 1.37E-10 1.32E-10 -5.99E-05
Abiotic depletion potential for fossil resources (ADPF) MJ 4.72E+01 4.45E+00 1.15E-01 6.5E-02 9E-03 -2.84E+01
m3 world eq
Water use (WDP) 8.44E-01 5.02E-04 4.5E-02 8.96E-06 2E-03 -6.51E-01
deprived
RESULTS OF THE LCA - INDICATORS TO DESCRIBE RESOURCE USE according to EN 15804+A2: DL200/300 Mortise Lock
Series
Parameter Unit A1-A3 A4 A5 C2 C3 D
Renewable primary energy as energy carrier (PERE) MJ 1.24E+01 1.1E-02 3.09E+00 2.04E-04 2E-03 -3.17E+00
Renewable primary energy resources as material utilization
MJ 3.07E+00 0 -3.07E+00 0 0 0
(PERM)
Total use of renewable primary energy resources (PERT) MJ 1.55E+01 1.1E-02 2.1E-02 2.04E-04 2E-03 -3.17E+00
Non renewable primary energy as energy carrier (PENRE) MJ 4.7E+01 4.45E+00 1.41E-01 6.5E-02 3.34E-01 -2.84E+01
Non renewable primary energy as material utilization (PENRM) MJ 3.51E-01 0 -2.6E-02 0 -3.25E-01 0
Total use of non renewable primary energy resources (PENRT) MJ 4.73E+01 4.45E+00 1.15E-01 6.5E-02 9E-03 -2.84E+01
Use of secondary material (SM) kg 2.94E-01 0 0 0 0 0
Use of renewable secondary fuels (RSF) MJ 0 0 0 0 0 0
Use of non renewable secondary fuels (NRSF) MJ 0 0 0 0 0 0
Use of net fresh water (FW) m3 3.4E-02 2.09E-05 1E-03 3.67E-07 4.66E-05 -2.4E-02
RESULTS OF THE LCA – WASTE CATEGORIES AND OUTPUT FLOWS according to EN 15804+A2:
DL200/300 Mortise Lock Series
Parameter Unit A1-A3 A4 A5 C2 C3 D
Hazardous waste disposed (HWD) kg 2.41E-07 4.25E-10 1.71E-10 6.29E-12 3.37E-11 -1.28E-06
Non hazardous waste disposed (NHWD) kg 2.02E-01 4.51E-04 1.2E-02 6.63E-06 2E-03 -1.4E-02
Radioactive waste disposed (RWD) kg 9.75E-04 3.69E-06 6.04E-06 6.96E-08 3.28E-07 -2.45E-04
Components for re-use (CRU) kg 0 0 0 0 0 0
Materials for recycling (MFR) kg 0 0 0 0 1.09E+00 0
Materials for energy recovery (MER) kg 0 0 0 0 0 0
Exported electrical energy (EEE) MJ 0 0 5.51E-01 0 0 0
Exported thermal energy (EET) MJ 0 0 1E+00 0 0 0
RESULTS OF THE LCA – additional impact categories according to EN 15804+A2-optional:
DL200/300 Mortise Lock Series
Parameter Unit A1-A3 A4 A5 C2 C3 D
Disease
Incidence of disease due to PM emissions (PM) 2.55E-07 4.21E-09 5.66E-10 2.4E-11 4.33E-11 -1.61E-07
incidence
Human exposure efficiency relative to U235 (IR) kBq U235 eq 1.21E-01 5.04E-04 9.33E-04 9.95E-06 2.96E-05 -1.6E-02
Comparative toxic unit for ecosystems (ETP-fw) CTUe 1.83E+01 3.16E+00 5.5E-02 4.6E-02 3E-03 -9.2E+00
Comparative toxic unit for humans (carcinogenic) (HTP-c) CTUh 4.3E-07 5.93E-11 2.9E-12 8.64E-13 2.87E-13 -2.47E-09
4 Environmental Product Declaration - dormakaba - DL 200/300
Comparative toxic unit for humans (noncarcinogenic) (HTP-nc) CTUh 6.04E-08 3.25E-09 1.27E-10 3.7E-11 2.91E-11 -1.94E-08
Soil quality index (SQP) SQP 5.43E+01 9E-03 3.1E-02 1.67E-04 3E-03 -2.47E+00
Disclaimer 1 – for the indicator “Potential Human exposure efficiency relative to U235”. This impact category deals mainly with the
eventual impact of low-dose ionizing radiation on human health of the nuclear fuel cycle. It does not consider effects due to possible
nuclear accidents, occupational exposure or radioactive waste disposal in underground facilities. Potential ionizing radiation from the
soil, radon and from some construction materials is also not measured by this indicator.
Disclaimer 2 – for the indicators “abiotic depletion potential for non-fossil resources”, “abiotic depletion potential for fossil resources”,
“water (user) deprivation potential, deprivation-weighted water consumption”, “potential comparative toxic unit for ecosystems”,
“potential comparative toxic unit for humans – cancerogenic”, “Potential comparative toxic unit for humans - not cancerogenic”,
“potential soil quality index”. The results of this environmental impact indicator shall be used with care as the uncertainties on these
results are high as there is limited experience with the indicator.
References
DIN 18251
DIN 18251:2020-04 - Locks - Mortise locks and multipoint GaBi
locks - Terms, definitions and dimensions Sphera Solutions GmbH Gabi Software System and Database
for Life Cycle Engineering 1992-2020 Version 10.0.0.71
EN 12209 University of Stuttgart Leinfelden-Echterdingen
EN 12209:2003 Building hardware – locks and latches –
mechanically operated locks, latches and locking plates – GaBi ts documentation
requirements and methods GaBi life cycle inventory data documentation (https://www.gabi-
software.com/support/gabi/gabidatabase- 2020-lci-
EN 15804 documentation/).
EN 15804 + A2:2019+A2+AC:2021 (in press), Sustainability of
construction works — Environmental Product Declarations — LCA-tool dormakaba
Core rules for the product category of construction products. LCA-tool: DHW.
Tool no.: IBU-DOR-202104-LT1-EN.
ISO 14025 Developed by Sphera Solutions GmbH
ISO 14025:2006;
Environmental labels and declarations — Type III PCR Part A
environmental declarations — Principles and procedures. PCR – Part A: Calculation Rules for the Life Cycle Assessment
and Requirements on the Project Re-port according to EN
Registration, Evalulation, Authorisation and Restriction of 15804+A2:2019, Version 1.0, 2020, Institut Bauen und Umwelt
Chemicals (REACH) e.V., www.ibu-epd.com.
Regulation (EC) No 1907/2006 of the European Parliament and
of the Council on the Registration, Evaluation, Authorisation PCR Part B
and Restriction of Chemicals (REACH). PCR – Part B: Requirements on the EPD for Building Hardware
product, version 1.2, Institut Bauen und Umwelt e.V., www.ibu-
Further References epd.com, 2017.
IBU 2021
General Instructions for the EPD programme of Institut Bauen
und Umwelt e.V.
Version 2.0, Berlin: Institut Bauen und Umwelt e.V., 2021.
www.ibu-epd.com
5 Environmental Product Declaration - dormakaba - DL 200/300
Publisher
Institut Bauen und Umwelt e.V. +49 (0)30 3087748- 0
Hegelplatz 1 info@ibu-epd.com
10117 Berlin www.ibu-epd.com
Germany
Programme holder
Institut Bauen und Umwelt e.V. +49 (0)30 3087748- 0
Hegelplatz 1 info@ibu-epd.com
10117 Berlin www.ibu-epd.com
Germany
Author of the Life Cycle Assessment
Sphera Solutions GmbH +49 711 341817-0
Hauptstraße 111- 113 info@sphera.com
70771 Leinfelden-Echterdingen www.sphera.com
Germany
Owner of the Declaration
dormakaba International Holding GmbH +49 2333 793-0
DORMA Platz 1 info.de@dormakaba.com
58256 Ennepetal www.dormakaba.com
Germany
6 Environmental Product Declaration - dormakaba - DL 200/300
