ENVIRONMENTAL-PRODUCT DECLARATION
as per ISO 14025 and EN 15804+A2
Owner of the Declaration Kingspan Insulation B.V.
Publisher Institut Bauen und Umwelt e.V. (IBU)
Programme holder Institut Bauen und Umwelt e.V. (IBU)
Declaration number EPD-KIN-20230010-CBD2-EN
Issue date 07.02.2023
Valid to 06.02.2028
Therma™ TF70
Kingspan Insulation B.V.
www.ibu-epd.com | https://epd-online.com
General Information
Kingspan Insulation B.V. Therma™ TF70
Programme holder Owner of the declaration
IBU – Institut Bauen und Umwelt e.V. Kingspan Insulation B.V.
Hegelplatz 1 Lingewei 8
10117 Berlin 4004LL Tiel
Germany Netherlands
Declaration number Declared product / declared unit
EPD-KIN-20230010-CBD2-EN Therma™ TF70
1m2, 120mm thickness, R = 5,45 m2.K/W
D
This declaration is based on the product category rules: Scope:
Insulating materials made of foam plastics, 08.03.2023 The insulation material Therma™ TF70 is produced by Kingspan Insulation
(PCR checked and approved by the SVR) at the manufacturing facilities in Winterswijk (the Netherlands),
Burkhardtsdorf (Germany) and Kankaanpää (Finland). This EPD is based
on
Issue date weighted averages which have been determined on
the basis of the single values originating from the different Kingspan
07.02.2023
Insulation factories.
Therma™ TF70 Floorboard is an insulation board with a rigid thermoset
polyisocyanurate (PIR) fibre-free insulation core, faced on both sides with
Valid to
a low emissivity composite foil. Therma™ TF70 Floorboard is used as
06.02.2028 thermal insulation for floors.
In order to enable the user of the EPD to calculate the LCA results for
different thicknesses, the EPD contains the respective calculation rules.
The owner of the declaration shall be liable for the underlying information
and evidence; the IBU shall not be liable with respect to manufacturer
information, life cycle assessment data and evidences.
The EPD was created according to the specifications of EN 15804+A2. In
the following, the standard will be simplified as EN 15804 bezeichnet.
Verification
Dipl.-Ing Hans Peters The standard EN 15804 serves as the core PCR
(chairman of Institut Bauen und Umwelt e.V.)
Independent verification of the declaration and data according to ISO
14025:2011
internally X externally
Dr. Alexander Röder Vito D'Incognito,
(Managing Director Institut Bauen und Umwelt e.V.) (Independent verifier)
1 Environmental-Product Declaration - Kingspan Insulation B.V. - Therma™ TF70
Product
Performance data of the product in accordance with the
Product description/Product definition declaration of performance with respect to its essential
Therma™ TF70 Floorboard is an insulation board with a rigid characteristics according to EN 13165 - Thermal insulation
thermoset polyisocyanurate (PIR) fibre-free insulation core, products for buildings - Factory made rigid polyurethane foam
faced on both sides with a low emissivity composite foil. The (PU) products - Specification
product is available in variable thicknesses from 20 mm up to The declaration of performance of the product can be found at
200 mm. This EPD is based on a thickness of 120 mm and www.kingspan.com.
R -value of 5,45 m²·K/W. For the placing on the market of the
D
Base materials/Ancillary materials
product in the European Union/European Free Trade
Association (EU/EFTA) (with the exception of Switzerland) The product contains approximately 3,3 kg/m2 polyurethane
Regulation (EU) No. 305/2011 (CPR) applies. The product rigid foam and 0,3 kg/m2 multi-layer aluminium facings.
needs a declaration of performance taking into consideration The main materials of the polyurethane foam are MDI (between
EN 13165 - Thermal insulation products for buildings - Factory 57-62 %), polyol (between 27-32 %) and a blowing agent
made polyurethane foam (PU) products - Specification and the (between 5-6 %). Due to the closed-cell structure (conform EN
CE-marking. For the application and use the respective national 13165), the blowing agent remains in the foam. Water, flame
provisions apply. retardants and additives are added (between 4-8 %).
In the current REACH regulations, polyurethane foam
Application insulation products are considered “articles” and are
Therma™ TF70 Floorboard is used as thermal insulation for exempt from the requirements of Articles 57 and 59(1)
floors. of REACH Regulation (EC) No 1907/2006. These
products are not classified as “hazardous products”
Technical Data
according to any current legislation, and can hence be
The technical specifications of the products within the scope of declared as follows:
the EPD shall be listed, including the reference to the test - This article contains substances listed in the
methods/test standards for each specification. candidate list (date: 31.08.2022) exceeding 0.1
percentage by mass: no.
For products with CE marking, the technical specifications must - This article contains other carcinogenic, mutagenic,
be specified in accordance with information in the declaration of reprotoxic (CMR) substances in categories 1A or 1B
performance. The properties relevant to the product should be which are not on the candidate list, exceeding 0.1
specified in the table below. If no information is given for percentage by mass: no.
properties, an explanation must be given in the background - Biocide products were added to this construction
report to the EPD as to why the property is not relevant to the product or it has been treated with biocide products
product. (this then concerns a treated product as defined by the
(EU) Biocidal Products Regulation No. 528/2012
Constructional data (BPR): no.
Name Value Unit
Environment and health during use
Thermal conductivity according to EN
0.022 W/(m.K)
13165 Reference service life
Reaction to fire according to EN The reference service life is not to be declared in this
E
13165 EPD as it does not cover the use stage.
Compressive strength according to CS(10\Y)
EN 13165 100/120
Thickness tolerance according to EN
T2-T3
13165
LCA: Calculation rules
manufacturing facilities in Winterswijk (the Netherlands),
Declared Unit Burkhardtsdorf (Germany) and Kankaanpää (Finland).
The declared unit (1 m²) and conversion factors are
listed in the table below. The environmental impacts have been calculated per plant over
Declared unit the calendar year 2021. Based on the one-year production
volume of Therma™ TF70 per plant, the individual
Name Value Unit
environmental impacts are weighted.
Declared unit 1 m2
Gross density 30 kg/m3 The EPD is studied for a common product thickness of 120
Grammage 3.6 kg/m2 mm. Multiplication factors are included to calculate impacts for
other product thicknesses within the range of 20 to 200 mm.
Layer thickness 0.12 m
This EPD is based on a weighted average of the annual For IBU core EPDs (where clause 3.6 is part of the EPD): for
production volume of three factories producing the products average EPDs, an estimate of the robustness of the LCA
Therma™ TF70. values must be made, e.g. concerning variability of the
production process, geographical representativeness and the
The scope of this EPD is the thermal insulation product influence of background data and preliminary products
Therma™ TF70 as produced by Kingspan Insulation at the compared to the environmental impacts caused by actual
2 Environmental-Product Declaration - Kingspan Insulation B.V. - Therma™ TF70
production. product
at the end-of-life stage are assigned to the product system
(C3); resulting potential credits for thermal and electrical energy
System boundary
from energy substitution are declared in module D.
The type of EPD according to EN 15804 is:
cradle to gate with options, modules C1–C4, and Geographic Representativeness
module D (A1–A3, C, D and additional modules: Land or region, in which the declared product system is
A4, A5). manufactured, used or handled at the end of the product´s
lifespan: Europe
The product stage is a mandatory information module and it
covers:
· A1, raw material extraction and processing, processing of Comparability
secondary material input (e.g. recycling processes), Basically, a comparison or an evaluation of EPD data is only
· A2, transport to the manufacturer, possible if all the data sets to be compared were created
· A3, manufacturing, including provision of all materials, according to EN 15804 and the building context, respectively
products and energy, packaging processing and its transport, the product-specific characteristics of performance, are taken
as well as waste processing up to the end-of-waste state or into account.
disposal of final residues
during the product stage. Background database
Background data from GaBi ts Version 10 is used with
The construction process stage includes: GaBi data sets CUP2022.1.
· A4 transport to the building site;
· A5 installation in the building including provision of all Factors for different thicknesses
materials, products and energy, as well as waste processing up The LCA results for the insulation material declared in
to the end-of-waste state or disposal of final residues during the this EPD refer to a product with a thickness of 120 mm.
construction process stage. To enable the user of the EPD to calculate the results for
different thicknesses the factors in the following
The end-of-life stage is a mandatory information module and it table can be used for the calculation. The LCA results in
covers: chapter 5 have to be
· C1 de-construction, demolition; multiplied by these factors.
· C2 transport to waste processing;
· C3 waste processing for reuse, recovery and/or recycling; The scaling factors are applicable for the complete
· C4 disposal (not applicable for this EPD) including provision product, where the multi-layer aluminium facings are
and all transport, provision of all materials, products and related for all product thicknesses equal and the foam inputs
energy and water use. are scaling upwards and downwards with other product
thicknesses.
Environmental burden of the incineration (R1 > 60 %) of the
LCA: Scenarios and additional technical information
Characteristic product properties are transported either on expanded polystyrene (EPS) skids or
Information on biogenic carbon on wooden
pallets.
The total mass of biogenic carbon containing materials is less Within Module A3 the following packaging of the final
than 5 % of the total mass of the product and accompanying product is included:
packaging. - Polyethylene cover and wrap: 0,052 kg/m²
Technical information - Expanded Polystyrene skid: 0,050 kg/m²
The following technical information is a basis for the - Wooden pallet: 0,000 kg/m²
declared modules or can be used for developing
Transport to the building site (A4)
specific scenarios in the context of a building
Name Value Unit
assessment.
Litres of fuel 0.0103 l/100km
Manufacturing (A3) Transport distance 100 km
A polyethylene packaging foil is used. The products Gross density of products transported 30 kg/m3
3 Environmental-Product Declaration - Kingspan Insulation B.V. - Therma™ TF70
Installation into the building (A5) End of life (C1-C4)
Name ValueUnit The assumptions for C1 are: diesel driven excavator (100 kW;
0.2 litre fuel per ton excavated material). The assumptions for
Total output substances following waste treatment
0.102 kg C2 are: Truck Euro 6, diesel driven, 26-28 t gross weight,
on-site packaging material
assumed distance 50 km
The recycling of the packaging is considered in A5.
Name ValueUnit
Collected as mixed construction waste 3.6 kg
In case a reference service life according to applicable ISO Energy recovery 3.575 kg
standards is declared then the assumptions and in-use Recycling (aluminium content of the multi-layer
0.025 kg
conditions underlying the determined RSL shall be declared. In aluminium facings)
addition, it shall be stated that the RSL applies for the reference
Reuse, recovery and/or recycling potentials (D), relevant
conditions only.
scenario information
Waste incineration with energy recuperation is assumed as an
The same holds for a service life declared by the manufacturer.
end-of-life scenario
Corresponding information related to in-use conditions needs
not be provided if a service life taken from the list on service life
by BNB is declared.
4 Environmental-Product Declaration - Kingspan Insulation B.V. - Therma™ TF70
LCA: Results
In Table 1 "Description of the system boundary", all declared modules shall be indicated with an "X"; all modules that are not declared
shall be indicated with "MND" (As default the modules B3, B4, B5 are marked as MNR – module not relevant). In the following tables,
columns can be deleted for modules that are not declared. Indicator values should be declared with three valid digits (eventually using
exponential form (e.g. 1,23E-5 = 0,0000123). A uniform format should be used for all values of one indicator.
If several modules are not declared and therefore have been deleted from the table, the abbreviations for the indicators can be
replaced by the complete names, while the readability and clear arrangement should be maintained; the legends can then be deleted.
If due to relevant data gaps, an indicator cannot be declared in a robust way, then the abbreviation “IND” (indicator not declared)
should be used for this indicator.
• 0 - calculated value is 0
• 0 - value falls under the cut-off
• 0 - assumption which exclude any flows (e.g. exported
electricity A1-A3)
• IND – in cases where the inventory does not support
the methodological approach or the calculation of the
specific indicator IND shall be used.
If no reference service life is declared (see chapter 2.13 "Reference Service Life"), the LCA results of the modules B1-B2 and B6-B7
shall refer to a period of one year. This shall then be indicated as an explanatory text below the tables. In addition, the formula for the
quantification of such B-modules over the total life cycle shall be provided.
DESCRIPTION OF THE SYSTEM BOUNDARY (X = INCLUDED IN LCA; ND = MODULE OR INDICATOR NOT DECLARED; MNR =
MODULE NOT RELEVANT)
BENEFITS
AND LOADS
CONSTRUCTION
BEYOND
PRODUCT STAGE PROCESS USE STAGE END OF LIFE STAGE
THE SYSTEM
STAGE
BOUNDARIE
S
la ire ta m w a Ry lp p u s tro p s n a rT g n iru tc a fu n a M e h t m o rf tro p s n a rTe tis e h t o t e ta g y lb m e s s A e s U e c n a n e tn ia M ria p e R tn e m e c a lp e R tn e m h s ib ru fe R y g re n e la n o ita re p Oe s u re ta w la n o ita re p Oe s u n o itc u rts n o c -e Dn o itilo m e d tro p s n a rT g n is s e c o rp e ts a W la s o p s iD -e s u e R-y re v o c e R-g n ilc y c e Rla itn e to p
A1 A2 A3 A4 A5 B1 B2 B3 B4 B5 B6 B7 C1 C2 C3 C4 D
X X X X X MND MND MNR MNR MNR MND MND X X X X X
RESULTS OF THE LCA - ENVIRONMENTAL IMPACT according to EN 15804+A2: 1m2 120mm Therma™ TF70
Parameter Unit A1-A3 A4 A5 C1 C2 C3 C4 D
GWP-total kg CO 2-Äq. 1.04E+01 3.02E-02 2.54E-01 2.3E-03 1.51E-02 7.79E+00 0 -3.23E+00
GWP-fossil kg CO 2-Äq. 1.06E+01 3.01E-02 2.54E-01 2.3E-03 1.5E-02 7.63E+00 0 -3.21E+00
GWP-biogenic kg CO 2-Äq. -2.33E-01 -4.16E-05 1.39E-05 3.08E-06 -2.08E-05 1.66E-01 0 -1.6E-02
GWP-luluc kg CO 2-Äq. 6.75E-03 1.68E-04 3.01E-06 2.84E-08 8.39E-05 1.43E-05 0 -3.67E-04
ODP kg CFC11-Äq. 2.75E-11 1.8E-15 4.52E-14 1.41E-16 9.01E-16 5.77E-13 0 -2.06E-11
AP mol H+-Äq. 2.21E-02 3.1E-05 3.16E-05 1.07E-05 1.55E-05 4.55E-03 0 -4.93E-03
EP-freshwater kg PO 4-Äq. 4.75E-05 8.98E-08 1.14E-08 4.64E-10 4.49E-08 1.56E-07 0 -4.24E-06
EP-marine kg N-Äq. 5.71E-03 1.01E-05 8.49E-06 5.09E-06 5.07E-06 2.2E-03 0 -1.19E-03
EP-terrestrial mol N-Äq. 5.89E-02 1.21E-04 1.44E-04 5.57E-05 6.04E-05 2.53E-02 0 -1.28E-02
kg NMVOC-
POCP 2.82E-02 2.73E-05 2.45E-05 1.44E-05 1.37E-05 5.64E-03 0 -3.37E-03
Äq.
ADPE kg Sb-Äq. 1.11E-05 2.52E-09 1.1E-09 9.41E-11 1.26E-09 1.58E-08 0 -4.7E-07
ADPF MJ 2.71E+02 4.02E-01 9.37E-02 3.11E-02 2.01E-01 2.02E+00 0 -5.38E+01
m3 world-Äq.
WDP 1.58E+00 2.7E-04 2.41E-02 4.27E-06 1.35E-04 7.72E-01 0 -3.53E-01
deprived
GWP = Global warming potential; ODP = Depletion potential of the stratospheric ozone layer; AP = Acidification potential of land and water; EP =
Eutrophication potential; POCP = Formation potential of tropospheric ozone photochemical oxidants; ADPE = Abiotic depletion potential for non-fossil
resources; ADPF = Abiotic depletion potential for fossil resources; WDP = Water (user) deprivation potential)
RESULTS OF THE LCA - INDICATORS TO DESCRIBE RESOURCE USE according to EN 15804+A2: 1m2 120mm Therma™
TF70
Parameter Unit A1-A3 A4 A5 C1 C2 C3 C4 D
PERE MJ 2.79E+01 2.29E-02 2.41E-02 1.18E-04 1.14E-02 3.54E-01 0 -1.53E+01
PERM MJ 0 0 0 0 0 0 0 0
PERT MJ 2.79E+01 2.29E-02 2.41E-02 1.18E-04 1.14E-02 3.54E-01 0 -1.53E+01
PENRE MJ 1.55E+02 4.03E-01 4.32E+00 3.12E-02 2.02E-01 1.14E+02 0 -5.38E+01
PENRM MJ 1.17E+02 0 -4.22E+00 0 0 -1.12E+02 0 0
5 Environmental-Product Declaration - Kingspan Insulation B.V. - Therma™ TF70
PENRT MJ 2.71E+02 4.03E-01 9.38E-02 3.12E-02 2.02E-01 2.02E+00 0 -5.38E+01
SM kg 0 0 0 0 0 0 0 0
RSF MJ 0 0 0 0 0 0 0 0
NRSF MJ 0 0 0 0 0 0 0 0
FW m3 7.3E-02 2.59E-05 5.72E-04 1.77E-07 1.29E-05 1.82E-02 0 -1.65E-02
PERE = Use of renewable primary energy excluding renewable primary energy resources used as raw materials; PERM = Use of renewable primary
energy resources used as raw materials; PERT = Total use of renewable primary energy resources; PENRE = Use of non-renewable primary energy
excluding non-renewable primary energy resources used as raw materials; PENRM = Use of non-renewable primary energy resources used as raw
materials; PENRT = Total use of non-renewable primary energy resources; SM = Use of secondary material; RSF = Use of renewable secondary fuels;
NRSF = Use of non-renewable secondary fuels; FW = Use of net fresh water
RESULTS OF THE LCA – WASTE CATEGORIES AND OUTPUT FLOWS according to EN 15804+A2:
1m2 120mm Therma™ TF70
Parameter Unit A1-A3 A4 A5 C1 C2 C3 C4 D
HWD kg 1.12E-07 1.93E-12 7.81E-12 1.03E-13 9.65E-13 2.76E-10 0 -6.66E-09
NHWD kg 2.84E-01 5.78E-05 2.28E-02 2.92E-06 2.89E-05 4.37E-02 0 -8.06E-02
RWD kg 3.13E-03 4.96E-07 3.9E-06 3.42E-08 2.48E-07 8.4E-05 0 -4.21E-03
CRU kg 0 0 0 0 0 0 0 0
MFR kg 0 0 0 0 0 2.54E-02 0 0
MER kg 0 0 1.02E-01 0 0 3.46E+00 0 0
EEE MJ 0 0 4.61E-01 0 0 1.32E+01 0 0
EET MJ 0 0 8.25E-01 0 0 2.36E+01 0 0
HWD = Hazardous waste disposed; NHWD = Non-hazardous waste disposed; RWD = Radioactive waste disposed; CRU = Components for re-use;
MFR = Materials for recycling; MER = Materials for energy recovery; EEE = Exported electrical energy; EET = Exported thermal energy
RESULTS OF THE LCA – additional impact categories according to EN 15804+A2-optional:
1m2 120mm Therma™ TF70
Parameter Unit A1-A3 A4 A5 C1 C2 C3 C4 D
Disease
PM 1.85E-07 1.79E-10 3.86E-10 1.21E-10 8.95E-11 1.27E-08 0 -4.29E-08
incidence
IR kBq U235-Äq. 3.71E-01 7.28E-05 5.36E-04 4.97E-06 3.64E-05 1.35E-02 0 -7.18E-01
ETP-fw CTUe 1.11E+02 2.79E-01 6.71E-02 2.17E-02 1.4E-01 6.96E-01 0 -1.22E+01
HTP-c CTUh 7.11E-09 5.63E-12 3.76E-12 4.01E-13 2.81E-12 5.21E-11 0 -6.32E-10
HTP-nc CTUh 6.04E-07 2.92E-10 3.81E-10 2.03E-11 1.46E-10 1.9E-09 0 -2.23E-08
SQP SQP 6.51E+01 1.38E-01 2.39E-02 8.58E-05 6.92E-02 4.26E-01 0 -9.27E+00
PM = Potential incidence of disease due to PM emissions; IR = Potential Human exposure efficiency relative to U235; ETP-fw = Potential comparative
Toxic Unit for ecosystems; HTP-c = Potential comparative Toxic Unit for humans (cancerogenic); HTP-nc = Potential comparative Toxic Unit for humans
(not cancerogenic); SQP = Potential soil quality index
Disclaimer 1 – for the indicator “Potential Human exposure efficiency relative to U235”.This impact category deals
mainly with the eventual impact of low-dose ionizing radiation on human health of the nuclear fuel cycle. It does
not consider effects due to possible nuclear accidents, occupational exposure or to radioactive waste disposal in
underground facilities. Potential ionizing radiation from the soil, radon and from some construction materials is
also not measured by this indicator.
Disclaimer 2 – for the indicators “abiotic depletion potential for non-fossil resources”, “abiotic depletion potential
for fossil resources”, “water (user) deprivation potential, deprivation-weighted water consumption”, “potential
comparative toxic unit for ecosystems”, “potential comparative toxic unit for humans – cancerogenic”, “Potential
comparative toxic unit for humans - not cancerogenic”, “potential soil quality index”. The results of this
environmental impact indicator shall be used with care as the uncertainties on these results are high as there is
limited experience with the indicator.
References
Biocidal Products Regulation No. 528/2012 (BPR)
Regulation (EU) No 528/2012 of the European EN 13165
Parliament and of the Council of 22 May 2012 EN 13165:2012+A2:2016: Thermal insulation products
concerning the making available on the market and for buildings. Factory made polyurethane foam (PU)
use of biocidal products products. Specification
CPR EN 15804
Regulation (EU) No. 305/2011 of the European EN 15804:2012+A2:2019+AC:2021, Sustainability of
Parliament and of the Council of 9 March 2011 laying construction works — Environmental Product
down harmonised condition for the marketing of Declarations — Core rules for the product category of
construction products and repealing Council Directive construction products.
89/106/EC
GaBi ts
ISO 14025 thinkstep AG: Leinfelden-Echterdingen GaBi Software-
EN ISO 14025:2011, Environmental labels and System and Database for Life Cycle Engineering 1992-
declarations — Type III environmental declarations — 2019
Principles and procedures.
6 Environmental-Product Declaration - Kingspan Insulation B.V. - Therma™ TF70
IBU 2021 Institut Bauen und Umwelt e.V., Berlin (pub.): Product
Institut Bauen und Umwelt e.V.: General Instructions Category Rules for Construction Products from the
for the EPD programme of Institut Bauen und Umwelt range of Environmental Product Declarations of Institut
e.V., Version 2.0, Berlin: Institut Bauen und Umwelt Bauen und Umwelt (IBU), Part B: Requirements on the
e.V., 2021. EPD for insulating materials made of foam
www.ibu-epd.com plastics. January 2019
LCA-tool REACH
Kingspan LCA tool, version 1.1. IBU-KSI-202001-LT1- Regulation (EC) No 1907/2006 of the European
EN. Parliament and of the Council on the Registration,
Developed by Sphera Solutions GmbH (formely Evaluation, Authorisation and Restriction of Chemicals
Thinkstep GmbH) (REACH)
https://echa.europa.eu/candidate-list-table;
PCR Version 1.7, Part A
Institut Bauen und Umwelt e.V., Berlin (pub.): Product Candidate list
Category Rules for Building-Related Products and https://echa.europa.eu/candidate-list-table; accessed
services, Part A: Calculation Rules for the Life Cycle 31.08.2022, 233 substances listed.
Assessment and Requirements on the Project Report The literature referred to in the Environmental Product
according to EN 15804+A2:2019 Declaration must be listed in full.Standards already fully quoted
November 2021 in the EPD do not need to be listed here again.
The current version of PCR Part A and PCR Part B of the PCR
PCR 2017, Part B document on which they are based must be referenced.
7 Environmental-Product Declaration - Kingspan Insulation B.V. - Therma™ TF70
Publisher
Institut Bauen und Umwelt e.V. +49 (0)30 3087748- 0
Hegelplatz 1 info@ibu-epd.com
10117 Berlin www.ibu-epd.com
Germany
Programme holder
Institut Bauen und Umwelt e.V. +49 (0)30 3087748- 0
Hegelplatz 1 info@ibu-epd.com
10117 Berlin www.ibu-epd.com
Germany
Author of the Life Cycle Assessment
Kingspan Insulation B.V. +31 (0) 543 543 210
Lingewei 8 info@kingspaninsulation.nl
4004LL Tiel www.kingspan.com
Netherlands
Owner of the Declaration
Kingspan Insulation B.V. +31 (0) 543 543 210
Lingewei 8 info@kingspaninsulation.nl
4004LL Tiel www.kingspan.com
Netherlands
8 Environmental-Product Declaration - Kingspan Insulation B.V. - Therma™ TF70
