ENVIRONMENTAL PRODUCT DECLARATION
as per ISO 14025 and EN 15804+A2
Owner of the Declaration Hammerer Aluminium Industries Santana S.R.L.
Publisher Institut Bauen und Umwelt e.V. (IBU)
Programme holder Institut Bauen und Umwelt e.V. (IBU)
Declaration number EPD-HAA-20230202-IBA1-EN
Issue date 15.09.2023
Valid to 14.09.2028
Aluminium billets 75PC
Hammerer Aluminium Industries Santana S.R.L.
www.ibu-epd.com | https://epd-online.com
1. General Information
Hammerer Aluminium Industries Santana Aluminium billets 75PC
S.R.L.
Programme holder Owner of the declaration
IBU – Institut Bauen und Umwelt e.V. Hammerer Aluminium Industries Santana S.R.L.
Hegelplatz 1 Calea Hammerer 5
10117 Berlin 317280 Santana
Germany Romania
Declaration number Declared product / declared unit
EPD-HAA-20230202-IBA1-EN The declared product is 1 kg of aluminium billets 75PC which consists of at
least 75 % post-consumer aluminium scrap.
This declaration is based on the product category rules: Scope:
Products of aluminium and aluminium alloys, 01.08.2021 This product declaration refers to a declared unit of 1 kg of aluminium
(PCR checked and approved by the SVR) billets 75PC produced in one production facility in Sântana, Romania.
The owner of the declaration shall be liable for the underlying information
and evidence; the IBU shall not be liable with respect to manufacturer
Issue date information, life cycle assessment data and evidences.
15.09.2023
The EPD was created according to the specifications of EN 15804+A2. In
the following, the standard will be simplified as EN 15804.
Valid to
Verification
14.09.2028
The standard EN 15804 serves as the core PCR
Independent verification of the declaration and data according to ISO
14025:2011
internally X externally
Dipl.-Ing. Hans Peters
(Chairman of Institut Bauen und Umwelt e.V.)
Florian Pronold Dr. Eva Schmincke,
(Managing Director Institut Bauen und Umwelt e.V.) (Independent verifier)
1 Environmental-Product Declaration - Hammerer Aluminium Industries Santana S.R.L. - Aluminium billets 75PC
2. Product
The main constituent of the aluminium billets is aluminium with
2.1 Product description/Product definition a share of around 99% and alloying metals in a percentage of
This EPD refers to 1 kg of aluminium billets 75PC consisting of around 1 %.
primary and recycled aluminium, reinforced by alloying
elements, with the internal code 75PC which means that at The share of aluminium in the product consists of about 20 %
least 75 % of the aluminium is post-consumer scrap. primary aluminium, at least 75 % post-consumer scrap and 4 %
The aluminium billets 75PC are sold under different names, pre-consumer scrap, while the rest of 1 % consists of alloys
depending on the customers' request. The names under which mixture.
the aluminium billets are sold are 6060PC and AS01. Based on
customers' request, the aluminium billets 75PC can be sold From the total amount of primary aluminium, HAI purchases
under different commercial names. around 71 % of it from a supplier that provides a low carbon
For the use and application of the product, the respective aluminium.
national provisions at the place of use apply.
The product/at least part of the product does not contain
2.2 Application
substances on the ECHA list of Substances of Very High
The final aluminium product (aluminium billets 75PC) is used Concern (SVHC) above 0.1 mass %.
for creating different aluminium products, for industry, building
and construction, and automotive industries. The aluminium The product/at least one sub-product does not contain other
billets 75PC are sold under different names, depending on the carcinogenic, mutagenic, reprotoxic (CMR) substances of
customers' request. The names under which the aluminium category 1A or 1B not on the candidate list above 0.1 mass %
billets are sold are 6060PC and AS01. Based on customers' in at least one sub-product.
request, the aluminium billets 75PC can be sold under different
commercial names.
No biocidal products have been added to the present
2.3 Technical Data
construction product or it has been treated with biocidal
The physical properties correspond to aluminium billets
products (it is thus a treated product within the meaning of the
products. The chemical composition of the aluminium billets is
Biocidal Products Regulation (EU) No 528/2012).
based on the EN AW-6060 specifications.
2.6 Manufacture
The final product has the characteristics described in the table The main technological flow in Hammerer Aluminium Industries
below. is the development of secondary aluminium by recycling
Constructional data aluminium waste in melting furnaces. The casting activity is
carried out in several stages, as follows:
Name Value Unit
Gross density 2700 kg/m3
Melting point 650 °C
Electrical conductivity at 20°C - m/Ωmm2
Thermal conductivity 220 W/(mK)
Coefficient of thermal expansion 23.4 10-6K-1
Modulus of elasticity 69500 N/mm2
Shear modulus 26100 N/mm2
Specific heat capacity 0.898 kJ/kgK
Specific heat capacity 0.898 kJ/kgK
Hardness 75 HB
Yield strength Rp 0,2 min. 160 N/mm2
Tensile strength Rm min. 215 N/mm2
Tensile stress at break 14 %
Note that the values for Hardness, Yield strength Rp 0,2 min.,
Tensile strength Rm min. and Tensile stress at break, are the
maximum ones. The mechanical properties after extrusion and
heat treatment, depend on temper. There are two production lines: Line 1, where aluminium waste
with high aluminium quantities is melted and casted in semi-
Performance data of the product with respect to its finished products and Line 2, where aluminium waste with lower
characteristics in accordance with the relevant technical aluminium quantities and dross (slag) is melted and casted. In
provision (no CE-marking). addition to that, aluminium ingots of primary aluminium are
delivered to the furnaces, where they are heated and mixed
2.4 Delivery status with secondary aluminium, originating from pre- and post-
The aluminium billets 75PC are delivered on the desired length consumer scrap and aluminium-rich waste from Line 2. The
and diameter. The most common length is 7 meters. The billets industrial products made are intended for the Business-to-
are secured during transport by being tied together using business market segment.
plastic bands and placed on rectangular wooden bars.
The company has implemented a certified quality management
2.5 Base materials/Ancillary materials system, IATF 16949, which monitors the entire manufacturing
process.
2 Environmental-Product Declaration - Hammerer Aluminium Industries Santana S.R.L. - Aluminium billets 75PC
used as inputs for different industries. Each industry might treat
2.7 Environment and health during manufacturing the aluminium based on the properties of the environment
The production facility has an environmental management where the finished products will stand. The treatment will
system in accordance with ISO 14001, an energy management influence the ageing of the final product.
in accordance with ISO 50001 and an occupational health and
safety management system in accordance with ISO 45001 in 2.13 Extraordinary effects
order to ensure environmental protection and occupational Fire
health and safety in the production process. Aluminium billets meet the requirements of building material
class A "non-combustible" according to DIN 4102-4.The melting
2.8 Product processing/Installation point of aluminium is approx. 650° C.
The aluminium billets are delivered to different industries and The toxicity of fire gases is not applicable.
the processing/installation depends on each individual industry.
Fire protection
Some of the processing activities of aluminium billets are, but
not limited to extrusion and forging. Name Value
Building material class A1
2.9 Packaging
Burning droplets Not applicable
The billets are tied together with plastic straps and placed on
Smoke gas development Not applicable
rectangular wooden bars. The number of billets tied together
and the length may differ, based on customers' requests.
Water
Both the wooden bars and the plastic straps can be recycled by The exposure of the aluminium billets to water does not alter
the customer. the product and has no negative impact on the environment
(water).
2.10 Condition of use
The aluminium billets are produced based on EN AW-6060 Mechanical destruction
specifications. Unforeseen mechanical destruction of the aluminium billets is
There are no special features of the material composition for not relevant.
the period of use.
2.14 Re-use phase
2.11 Environment and health during use The aluminium billets are 100 % recyclable. The material does
If the aluminium billets are used as intended, no hazards to air, not suffer any loss of quality and can be recycled forever. The
water and soil as well as to human health can arise. scrap resulting in the production process is processed into new
aluminium billets.
No harmful substances are incorporated in the product. The aluminium scrap from demolition can be separated,
collected and recycled by the recycling industry.
The environmental impact during the use phase depends on
the design of the end product since aluminium billets are not 2.15 Disposal
finished products. According to the European Waste Catalog (EWC), the disposal
code depends on the end product.
2.12 Reference service life Given its high value, the aluminium scrap it's not disposed but
The aluminium billets are not a final product and they are used used as a raw material in the recycling industry.
for different industries as input material where it can have
multiple applications, therefore no reference service life (RSL) 2.16 Further information
is declared for aluminium billets. For more information, visit: https://www.hai-aluminium.com/
The aluminium billets are not a finished product and they are
3. LCA: Calculation rules
The LCA for aluminium billets is a cradle-to-gate assessment of
3.1 Declared Unit the environmental impacts with options.
The declared unit refers to 1 kg of aluminium billets 75PC, from The following life cycle phases are considered in the analysis:
a single major production line (Remelting and Casting). The Module A1-A3 | Product stage
product consists of primary and recycled aluminium (99 %), The following processes were considered:
reinforced by alloying elements (~1 %). There are no by-
• The purchase of the raw materials and the ancillary
products formed from the production line subject to this study.
materials such as primary aluminium, recycled
The aluminium billets 75PC consist of at least 75 % post-
aluminium as well as ancillary materials such as alloying
consumer scrap, 20 % virgin aluminium, 4 % of pre-consumer
metals and packaging.
scrap and the rest of 1 % alloying metals.
• The transport of the raw and ancillary materials was
Declared unit and mass reference calculated based on the actual distances of the
Name Value Unit suppliers.
• The energy consists of diesel used in the manufacturing
Declared unit 1 kg
process and natural gas which is supplied from the
national grid.
Data used in calculations represent site-specific production • The electricity is 100 % green electricity based on the
volumes for 2022 of the main product line as well as calculated contract concluded between HAI and the electricity
data based on the share of the product in the total production. supplier.
The share used, is presented in the Assumptions chapter. Module C2 | Transport to waste processing
Module C2 declares the environmental impacts resulting from
3.2 System boundary
transporting the waste aluminium to a waste processing facility
at an assumed distance of 50 km.
3 Environmental-Product Declaration - Hammerer Aluminium Industries Santana S.R.L. - Aluminium billets 75PC
All inputs and outputs from background system to foreground
Module C3 | Waste processing system processes, with significant potential impact, are
Module C3 declares the environmental impacts resulting from included in the calculation, as company specific data is
the treatment of aluminium scrap by collecting, sorting, cleaning available. Cut-off criteria are set to be not more than 1% of
and pressing (90 % of the product). renewable and non-renewable primary energy usage and not
more than 1% of the total mass flow for a single flow and 99%
Module C4 | Disposal of all flows are considered.
Module C4 declares the environmental impacts resulting from
landfilling (10 % of the product). 3.5 Background data
Calculations were performed using Simapro 9.4.0.2, where
Module D | Credits and loads outside the system boundary inputs and outputs are listed. The LCA impacts were calculated
In Module D, the substitution potential of primary aluminium using characterization factors from Ecoinvent 3.8 database,
through a recycling scenario (90 % of the product) is presented. applying the EN 15804 + A2 Method V1.03 / EF 3.0
normalization and weighting set.
3.3 Estimates and assumptions
This study analysis is based mainly on on-site specific data 3.6 Data quality
related to product manufacturing. Study results are valid for the Data reliability is ensured by the manufacturer's data
technological process specified, geographical area and time management systems and expert knowledge of plant
period mentioned. engineers. Additional questions regarding reported values (e.g.,
Furthermore, the following estimates have been made: type of material, materials use, waste management techniques,
transportation distances, etc.) were answered and clarified by
• Alloys – for the purpose of calculations all alloys are
plant engineers.
assumed to
be pure substances, thus containing 100 % of a given
3.7 Period under review
substance (e.g. Mg, Zn). The alloys contribute about 1
Site-specific data is collected for all flows according to the set
% to the final product.
cut-off criteria. Data collected is representative of one and the
• It was assumed that soft sawn wood with a density of
same technology for the period between the 1st of January
540 kg/m3 is used for wood packaging.
2022 to the 31st of December 2022. All the collected data is
• The use of Euro 6 trucks is assumed for the transport,
based on the actual quantities used and produced during this
due to the prevalence of this type of Euro trucks in the
period.
fleet transporting materials.
• For all inputs a dataset representative for the European 3.8 Geographic Representativeness
market was selected (if available) or a global market
Land or region, in which the declared product system is
dataset in case a European dataset was not available.
manufactured, used or handled at the end of the product´s
• Only the environmental burden from collection, sorting
lifespan: Europe
and transportation of Al scrap used as an input is
accounted for.
• All waste outputs such as mixed plastic, wood, 3.9 Allocation
cardboard, are accounted for by selecting datasets In this study there are no by-products and thus no relevant
representative for the market, where transport is already allocation is considered necessary since all inputs are
included in the final assessment of the impacts. converted to the main product described above and waste
Respective types of waste treatment have been outflows.
selected (preparation for recycling, incineration, The total environmental burden is associated with the products
landfilling). delivered to the customers
• The amount of used water is accounted as tap water
from municipal supply or underground water without 3.10 Comparability
treatment depending on the reported quantities. Basically, a comparison or an evaluation of EPD data is only
• The manufacturing process of the 75PC aluminium possible if all the data sets to be compared were created
billets is identical with the manufacturing process of the according to EN 15804 and the building context, respectively
other alloys, therefore a share of 0.2913 % was used for the product-specific characteristics of performance, are taken
alloys consumption and a share of 0.2629 % was used into account.
for the rest of the inputs, such as energy, fuels, waste. Calculations were performed using Simapro 9.4.0.2, where
The share was calculated based on the mass of the inputs and outputs are listed. The LCA impacts were calculated
75PC production against total plant production. using characterization factors from Ecoinvent 3.8 database.
3.4 Cut-off criteria
4. LCA: Scenarios and additional technical information
Association.
Characteristic product properties biogenic carbon
Name Value Unit
Biogenic carbon is present only in the wooden packaging and it
Recycling 0.9 kg
is not reported since the wood packaging represents less than
1 % from the total inputs of packaging. Landfilling 0.1 kg
Reuse, recovery and/or recycling potentials (D), relevant
End of life (C1-C4) scenario information
For the end-of-life scenario used in this study the following
Name Value Unit
assumptions and thus follows the most recent data on
Recycling 90 %
aluminium recycling published by the European Aluminium
4 Environmental-Product Declaration - Hammerer Aluminium Industries Santana S.R.L. - Aluminium billets 75PC
5. LCA: Results
The following table shows the LCA results for the declared unit of 1 kg of aluminium billets.
DESCRIPTION OF THE SYSTEM BOUNDARY (X = INCLUDED IN LCA; ND = MODULE OR INDICATOR NOT DECLARED; MNR =
MODULE NOT RELEVANT)
Benefits and
Construction loads beyond
Product stage Use stage End of life stage
process stage the system
boundaries
la ire ta m w a Ry lp p u s tro p s n a rT g n iru tc a fu n a M e h t m o rf tro p s n a rTe tis e h t o t e ta g y lb m e s s A e s U e c n a n e tn ia M ria p e R tn e m e c a lp e R tn e m h s ib ru fe R y g re n e la n o ita re p Oe s u re ta w la n o ita re p Oe s u n o itc u rts n o c -e Dn o itilo m e d tro p s n a rT g n is s e c o rp e ts a W la s o p s iD -e s u e R-y re v o c e R-g n ilc y c e Rla itn e to p
A1 A2 A3 A4 A5 B1 B2 B3 B4 B5 B6 B7 C1 C2 C3 C4 D
X X X MND MND MND MND MNR MNR MNR MND MND MND X X X X
RESULTS OF THE LCA - ENVIRONMENTAL IMPACT according to EN 15804+A2: 1 kg aluminium billets
Parameter Unit A1-A3 C2 C3 C4 D
Global Warming Potential total (GWP-total) kg CO 2 eq 1.74E+00 1.07E-02 2.4E-01 5.56E-03 -1.63E+00
Global Warming Potential fossil fuels (GWP-fossil) kg CO 2 eq 1.7E+00 1.07E-02 2.38E-01 5.52E-03 -1.59E+00
Global Warming Potential biogenic (GWP-biogenic) kg CO 2 eq 1.99E-03 1.03E-05 1.72E-03 3.92E-05 -5.45E-03
Global Warming Potential luluc (GWP-luluc) kg CO 2 eq 3.48E-02 5.04E-06 3.2E-04 5.09E-06 -3.12E-02
Depletion potential of the stratospheric ozone layer (ODP) kg CFC11 eq 1.27E-07 2.41E-09 1.11E-08 7.62E-10 -1.11E-07
Acidification potential of land and water (AP) mol H+ eq 1.77E-02 3.02E-05 9.57E-04 3.4E-05 -1.22E-02
Eutrophication potential aquatic freshwater (EP-freshwater) kg P eq 1.8E-04 8.05E-07 6.74E-05 1.3E-06 -7.24E-04
Eutrophication potential aquatic marine (EP-marine) kg N eq 2.35E-03 5.9E-06 1.35E-04 9.08E-06 -1.61E-03
Eutrophication potential terrestrial (EP-terrestrial) mol N eq 1.95E-02 6.42E-05 1.49E-03 9.81E-05 -1.6E-02
kg NMVOC
Formation potential of tropospheric ozone photochemical oxidants (POCP) 6.24E-03 2.46E-05 4.28E-04 2.93E-05 -5.34E-03
eq
Abiotic depletion potential for non fossil resources (ADPE) kg Sb eq 5.67E-06 4.88E-08 1.1E-05 1.39E-08 1.33E-05
Abiotic depletion potential for fossil resources (ADPF) MJ 2.44E+01 1.6E-01 1.56E+00 7.88E-02 -2E+01
m3 world eq
Water use (WDP) 3.78E-01 5.3E-04 2.02E-02 1.53E-03 -2.54E-01
deprived
RESULTS OF THE LCA - INDICATORS TO DESCRIBE RESOURCE USE according to EN 15804+A2: 1 kg aluminium billets
Parameter Unit A1-A3 C2 C3 C4 D
Renewable primary energy as energy carrier (PERE) MJ 1.17E+01 2.7E-03 2.09E-01 4.05E-03 -7.64E+00
Renewable primary energy resources as material utilization (PERM) MJ 7.74E-03 0 0 0 0
Total use of renewable primary energy resources (PERT) MJ 1.17E+01 2.7E-03 2.09E-01 4.05E-03 -7.64E+00
Non renewable primary energy as energy carrier (PENRE) MJ 2.44E+01 1.6E-01 1.57E+00 7.88E-02 -2E+01
Non renewable primary energy as material utilization (PENRM) MJ 0 0 0 0 0
Total use of non renewable primary energy resources (PENRT) MJ 2.44E+01 1.6E-01 1.57E+00 7.88E-02 -2E+01
Use of secondary material (SM) kg 8.46E-01 0 0 0 0
Use of renewable secondary fuels (RSF) MJ 0 0 0 0 0
Use of non renewable secondary fuels (NRSF) MJ 0 0 0 0 0
Use of net fresh water (FW) m3 2.29E-03 0 0 0 0
RESULTS OF THE LCA – WASTE CATEGORIES AND OUTPUT FLOWS according to EN 15804+A2:
1 kg aluminium billets
Parameter Unit A1-A3 C2 C3 C4 D
Hazardous waste disposed (HWD) kg 2.93E-05 4.28E-07 5.94E-03 1.15E-07 2.25E-04
Non hazardous waste disposed (NHWD) kg 6.85E-01 6.79E-03 1.38E-01 2.06E-01 -4.39E-01
Radioactive waste disposed (RWD) kg 1.46E-04 1.07E-06 6.49E-06 3.72E-07 -8.05E-05
Components for re-use (CRU) kg 0 0 0 0 0
Materials for recycling (MFR) kg 1.22E-03 0 0 0 0
Materials for energy recovery (MER) kg 0 0 0 0 0
Exported electrical energy (EEE) MJ 0 0 0 0 0
Exported thermal energy (EET) MJ 0 0 0 0 0
RESULTS OF THE LCA – additional impact categories according to EN 15804+A2-optional:
1 kg aluminium billets
Parameter Unit A1-A3 C2 C3 C4 D
Disease
Incidence of disease due to PM emissions (PM) 2.7E-07 7.29E-10 1.47E-08 5.86E-10 -1.29E-07
incidence
Human exposure efficiency relative to U235 (IR) kBq U235 eq 3.8E-01 8.49E-04 1.61E-02 4.5E-04 -2.2E-01
Comparative toxic unit for ecosystems (ETP-fw) CTUe 4.48E+01 4.61E-02 5.68E-01 1.58E-01 -1.96E+01
Comparative toxic unit for humans (carcinogenic) (HTP-c) CTUh 8.55E-09 2.18E-12 5.04E-11 2.82E-12 -4.19E-09
Comparative toxic unit for humans (noncarcinogenic) (HTP-nc) CTUh 7.63E-08 1.26E-10 6.93E-09 1.14E-10 -5.89E-08
5 Environmental-Product Declaration - Hammerer Aluminium Industries Santana S.R.L. - Aluminium billets 75PC
Soil quality index (SQP) SQP 5.15E+00 9.45E-02 1.49E+00 9.88E-02 -1.15E+00
Disclaimer 1 – for the indicator “Potential Human exposure efficiency relative to U235”. This impact category deals mainly with the
eventual impact of low-dose ionizing radiation on human health of the nuclear fuel cycle. It does not consider effects due to possible
nuclear accidents, occupational exposure nor due to radioactive waste disposal in underground facilities. Potential ionizing radiation
from the soil, from radon and from some construction materials is also not measured by this indicator.
Disclaimer 2 – for the indicators “abiotic depletion potential for non-fossil resources”, “abiotic depletion potential for fossil resources”,
“water (user) deprivation potential, deprivation-weighted water consumption”, “potential comparative toxic unit for ecosystems”,
“potential comparative toxic unit for humans – cancerogenic”, “Potential comparative toxic unit for humans - not cancerogenic”,
“potential soil quality index”. The results of this environmental impact indicator shall be used with care as the uncertainties on these
results are high or as there is limited experienced with the indicator.
6. LCA: Interpretation
The LCA results are presented for 1 kg of aluminium billets In the figure below it can be seen that by excluding the final
75PC. The charts below provide information on the impacts per disposal materials still represent the dominant category and are
main processes of the upstream and manufacturing life cycle responsible for 80 % of the total climate change impact
stages. There are no known limitations to the results in the category.
context of the set goal and scope of the study.
Based on the results it can be concluded that the dominant
material category appears to be materials responsible for 79.56
% for climate change category. The second biggest contributor
to the overall impact is energy with 14.71 % for climate change
category followed by transportation with a contribution of 5.27
% for climate change category.
7. Requisite evidence
The product is not a finished product (end product) and it is the design of the end product will vary, depending on the
used as raw material for other industries. The processing and application of the final product.
8. References
Standards ISO 14040:2006, Environmental management — Life cycle
assessment — Principles and framework
DIN EN 573-3:2019-10
Aluminium and aluminium alloys - Chemical composition and ISO 14044
form of wrought products - Part 3: Chemical composition and ISO 14044:2006, Environmental management — Life cycle
form of products assessment — Requirements and guidelines
DIN 4102-4 EN 15804
Fire behaviour of building materials and building components - EN 15804:2012+A2:2019+AC:2021, Sustainability of
Part 4: Synopsis and application of classified building materials, construction works — Environmental Product Declarations —
components and special components Core rules for the product category of construction products.
IATF 16949 ISO 45001
IATF 16949:2016 Quality management system for ISO 45001:2018 Occupational health and safety management
organizations in the automotive industry systems
ISO 14001
ISO 14001:2015 Environmental management systems ISO 50001
ISO 50001:2018 Energy management systems
ISO 14025 Further References
EN ISO 14025:2011, Environmental labels and declarations —
Type III environmental declarations — Principles and BPR Regulation
procedures. Biocidal Products Regulation EU 528/2012
ISO 14040 European Aluminium Association
6 Environmental-Product Declaration - Hammerer Aluminium Industries Santana S.R.L. - Aluminium billets 75PC
A strategy for achieving aluminium's full potential for circular epd.com
economy by 2030
https://european-aluminium.eu/wp- PCR Part A: Calculation Rules for the Life Cycle Assessment
content/uploads/2022/08/european-aluminium-circular- and Requirements on the Project Report according to EN
aluminium-action-plan.pdf 15804+A2:2019, v. 1.3
ECHA list PCR Part B: Requirements on the EPD for Products of
List of substances of very high concern (SVHC) for aluminium and aluminium alloys, v. 1.6
authorisation (ECHA Candidate List), 14.01.2020, published
under Article 59(10) of REACH. Helsinki: European Chemicals Software and database
Agency. http://echa.europa.eu/
European Waste Catalogue (EWC) SimaPro
Ordinance on the European Waste List (Waste List Ordinance LCA and reporting softwareapps.simapro.com
AVV)
ecoinvent Version 3
IBU Wernet, G., Bauer, C., Steubing, B., Reinhard, J., Moreno-Ruiz,
Institut Bauen und Umwelt e.V.: General Instructions for the E., and Weidema, B., 2016. The ecoinvent database version 3
EPD programme of Institut Bauen und Umwelt e.V., Version (part I): overview and methodology. The International Journal of
2.0, Berlin: Institut Bauen und Umwelt e.V., 2021, www.ibu- Life Cycle Assessment, [online] 21(9), pp.1218–1230.
7 Environmental-Product Declaration - Hammerer Aluminium Industries Santana S.R.L. - Aluminium billets 75PC
Publisher
Institut Bauen und Umwelt e.V. +49 (0)30 3087748- 0
Hegelplatz 1 info@ibu-epd.com
10117 Berlin www.ibu-epd.com
Germany
Programme holder
Institut Bauen und Umwelt e.V. +49 (0)30 3087748- 0
Hegelplatz 1 info@ibu-epd.com
10117 Berlin www.ibu-epd.com
Germany
Author of the Life Cycle Assessment
denkstatt Bulgaria OOD +359 2 470 7508
Lyubata 4-6 office@denkstatt.bg
1407 Sofia http://denkstatt.bg/
Bulgaria
Owner of the Declaration
Hammerer Aluminium Industries Santana S.R.L. +40 751 078 857
Calea Hammerer 5 Andreia.Godea@hai-
317280 Santana aluminium.com
Romania www.hai-aluminium.com
8 Environmental-Product Declaration - Hammerer Aluminium Industries Santana S.R.L. - Aluminium billets 75PC
