ENVIRONMENTAL PRODUCT DECLARATION
as per ISO 14025 and EN 15804+A2
Owner of the Declaration VELUX Group
Publisher Institut Bauen und Umwelt e.V. (IBU)
Programme holder Institut Bauen und Umwelt e.V. (IBU)
Declaration number EPD-VEL-20230281-IBA2-EN
Issue date 21.08.2023
Valid to 20.08.2028
VELUX sun tunnel TCF for flat roof, flexible, acrylic dome
VELUX A/S
www.ibu-epd.com | https://epd-online.com
1. General Information
VELUX A/S VELUX sun tunnel TCF for flat roof, flexible,
acrylic dome
Programme holder Owner of the declaration
IBU – Institut Bauen und Umwelt e.V. VELUX Group
Hegelplatz 1 Ådalsvej 99
10117 Berlin 2970 Hørsholm
Germany Denmark
Declaration number Declared product / declared unit
EPD-VEL-20230281-IBA2-EN The declaration represents 1 piece of VELUX sun tunnel TCF for flat roof,
flexible, with an acrylic dome.
This declaration is based on the product category rules: Scope:
Windows and doors , 01.08.2021 The declaration covers 100% of VELUX sun tunnel TCF for flat roof,
(PCR checked and approved by the SVR) flexible, with an acrylic dome by Partizánske Building Components SK,
Slovakia.
Issue date The owner of the declaration shall be liable for the underlying information
and evidence; the IBU shall not be liable with respect to manufacturer
21.08.2023
information, life cycle assessment data and evidences.
The EPD was created according to the specifications of EN 15804+A2. In
Valid to
the following, the standard will be simplified as EN 15804.
20.08.2028
Verification
The standard EN 15804 serves as the core PCR
Independent verification of the declaration and data according to ISO
14025:2011
internally X externally
Dipl.-Ing. Hans Peters
(Chairman of Institut Bauen und Umwelt e.V.)
Florian Pronold Dr. Matthew Fishwick,
(Managing Director Institut Bauen und Umwelt e.V.) (Independent verifier)
1 Environmental Product Declaration - VELUX A/S - VELUX sun tunnel TCF for flat roof, flexible, acrylic dome
2. Product
Composition of the sun tunnel TCF 0K14 0010:
2.1 Product description/Product definition Polyvinyl chloride (PVC) 50%
The VELUX flexible sun tunnel TCF is used for installation in Acrylonitrile Butadiene Styrene (ABS) 17%
flat roofs which brings natural light into areas of the house Poly(methyl methacrylate) (PMMA) 13%
where a flat-roof window installation is either not possible or not Polycarbonate 9%
appropriate. Ethylene propylene diene monomer (EPDM) 3%
The frame is made of white polyvinyl chloride (PVC). Sash and Stainless steel 2%
diffuser are made of acrylonitrile styrene acrylate (ASA) plastic Aluminium 1%
and the dome is made of transparent plastic (acrylate). The Zinc alloy 1%
tunnel is made of flexible reflective material. Steel 1%
Others 3%
For the placing of the product on the market in the European
Union/European Free Trade Association (EU/EFTA) (with the 1) 'This product/article/at least one partial article contains
exception of Switzerland) the Regulation (EU) No. 305/2011/ substances listed in the ECHA candidate list (date: 02.03.2022)
(CPR) applies. The product needs a declaration of performance exceeding 0.1 percentage by mass:
in accordance with the CPR taking into the European Technical
• no
Assessment: ETA -13/0764 of 14/10/2015. The CE-marking for
2) 'This product/article/at least one partial article contains other
the product takes into account the Declaration of Performance
carcinogenic, mutagenic, or toxic for reproduction (CMR)
in accordance with the CPR. For the application and use the
substances in categories 1A or 1B which are not on the ECHA
respective national provisions apply.
candidate list, exceeding 0.1 percentage by mass:
2.2 Application • not investigated with suppliers
The sun tunnel for flat roofs can be installed in roof pitches 3) 'Biocide products were added to this construction product or
between 0° and 15°. The sun tunnel is applicable to flat roofing it has been treated with biocide products (this then concerns a
materials. It can be integrated in roofing felt, roofing treated product as defined by the (EU) Regulation on Biocidal
membranes and in fully supported zinc or copper metal roofing. Products No. 528/2012):
• no
2.3 Technical Data
The Declaration of Performance including relevant technical
specifications and test methods/test standards can be
Recycled content
downloaded from the website www.velux.com/ce.
Constructional data for TCF 0K14 0010
For other variants, see velux.com/ce
Name Value Unit
Reaction to fire E class
Resistance to upward load EN 1875 UL 1500 -
The values stated in the table relate to the recycled material
water permeability acc. to EN 13985, EN - class streams in VELUX production.
1027
Resistance to downward load EN 1873 UL 2500 - 2.6 Manufacture
A few components are produced/processed internally. The
Resistance to fire EN 13501-2 NPD -
majority of products are bought from external suppliers and
External fire performance EN 13501-5 NPD -
assembled into the final product.
Water tightness EN 1873 9A -
Impact resistance - small hard body passed The factory is ISO 9001 certified.
NPD -
EN 1873
2.7 Environment and health during manufacturing
Impact resistance - large soft body EN 1873 NPD -
The factory is ISO14001 and ISO 45001 certified.
Direct airborne sound insulation EN ISO 54 (-5;-
dB
410-3 7)
2.8 Product processing/Installation
Thermal transmittance EN 1873 2.5 W/(m2K) The sun tunnel is fitted directly to the roof with the screws
Luminous transmittance EN 410 NPD - supplied.
Air permeability EN 1026 3 Class It is important that frame and roofing material are fitted
according to the installation instructions. Distance from interior
Durability EN 1873 passed -
ceiling finish to the upper edge of battens (measured in the
Performance data of the product in accordance with the centre of the tunnel): 0.2 - 0.9 m
declaration of performance with respect to its essential Installation of a sun tunnel requires access to the attic and the
characteristics according to ETA -13/0764 of 14/10/2015. roof.
Performance data of the product, based on the harmonised
standards, in accordance with the other provisions for 2.9 Packaging
harmonization. The packaging usually consists of:
- cardboard
2.4 Delivery status
- paper
The product is available in a diameter of 350 mm. - polyethylene film
- polystyrene foam parts
- steel
2.5 Base materials/Ancillary materials
2 Environmental Product Declaration - VELUX A/S - VELUX sun tunnel TCF for flat roof, flexible, acrylic dome
The use of other packaging materials is possible, but
insignificant in terms of quantity.
The plastic packaging (polyethylene (PE) film, polystyrene foam Water
parts), paper and cardboard as well as steel can be recycled if In the event of unforeseen exposure to water (flood), no
separated by type; alternatively, they - except steel - can be adverse effects on human health or the environment are to be
incinerated. expected.
Mechanical destruction
In the event of unforeseen mechanical destruction, VELUX sun
2.10 Condition of use tunnels have to be replaced; apart from potential injuries from
The material composition of VELUX sun tunnels does not sharp edges, no adverse effects on human health or the
change over their service life. environment are to be expected.
2.11 Environment and health during use 2.14 Re-use phase
VELUX sun tunnels do not contain any pollutants that could be VELUX sun tunnels can be dismantled manually without any
released during use. problems. The metal parts are usually recycled, and the plastic
parts are sent for thermal recycling for energy recovery.
Environmental protection: According to current knowledge, Tempered glass can be recycled.
hazards to water, air and soil cannot arise when the products
are used as intended. 2.15 Disposal
VELUX sun tunnels are mostly inert and can be disposed of in
Health protection: According to current knowledge, no health an appropriate landfill. However, due to the value of the
hazards or impairments are to be expected. materials or the carbon content of the plastic parts, recycling or
energy recovery is preferable and common.
2.12 Reference service life
It is not possible to calculate the reference service life Waste code according to the European Waste List (Regulation
according to ISO 15686. The service life based on a on the European Waste List):
manufacturer's declaration is 30 years. The corresponding 17 02 02 glass
utilization scenario is declared in 4. 17 02 03 plastics
17 04 14 mixed metals
2.13 Extraordinary effects
Fire 2.16 Further information
Fire performance according to EN 13501-1 Further documentation on the products, technical data sheets,
BIM files, etc. can be found at:
Name Value
www.velux.com
Building material class B
Burning droplets s1
Smoke gas development d0
3. LCA: Calculation rules
3.1 Declared Unit Module A5: The products are delivered to the construction site
The declared unit is 1 piece of VELUX sun tunnel TCF for flat ready to be installed. Manual installation is assumed; electricity
roof, flexible with an acrylic dome (TCF 0K14 0010) for a consumption related to electric drilling machines, screwdrivers,
diameter of 350 mm. etc. is considered to be negligible. The combustible packaging
Declared unit material (plastics) is assumed to be thermally treated in a
municipal waste incineration plant with an efficiency R1 < 0.6
Name Value Unit
(according to the ecoinvent v3.8 (cut-off) dataset used); the
Declared unit 1 piece
recovered energy is declared as exported energy. Metals,
Area 0.1225 m² paper and cardboard are recycled; it is assumed that these
Mass reference 9.29 kg/pce fractions reach the end-of-waste state after having been sorted
and transported (as a conservative choice) to a recycler. No
packaging waste is landfilled.
3.2 System boundary
Modules B1 to B7 are not relevant for the product under
Type of EPD: Cradle to gate with options, with modules C1 –
consideration or no significant environmental impacts occur.
C4, and module D (A1-A3, C, D and additional modules)
Module C1 includes manual dismantling, with no significant
The production of VELUX sun tunnels (modules A1-A3)
environmental impact.
includes raw material extraction, energy generation, waste
treatment and all transports up to the factory gate. In
Module C2 comprises the transport of the dismantled VELUX
accordance with COUNCIL REGULATION (EU) No 333/2011,
sun tunnel to a sorting plant and then to a waste incineration
secondary metals are modelled as part of the product system
plant for the thermally treated plastic fraction.
from the moment they are available as unmixed scrap.
Waste or secondary fuels are not used for production.
Modules C3/C4: given the complexity of the inventoried
products, a mixed end-of-life scenario is modelled, allowing the
Module A4 is not declared due to large variances in transport
different materials to follow their most likely path.
distances between the production site and the construction site,
As a rule of thumb, metals are recycled and plastics are
where the product is installed.
3 Environmental Product Declaration - VELUX A/S - VELUX sun tunnel TCF for flat roof, flexible, acrylic dome
incinerated (also due to the very limited data available on fully linked with corresponding data records from the
plastics recycling and its benefits); for metals it is assumed that background database ecoinvent v3.8 (cut-off).
these fractions reach the end-of-waste state after having been The background data was updated in 2021. Thus, the quality of
sorted and transported to a recycler. The combustible material the foreground and background data can be rated as very
(plastics, etc.) is assumed to be thermally treated in a municipal good.
waste incineration plant.
3.7 Period under review
Module D includes the benefits and burdens associated with The LCA data represents the production conditions for the year
recycling metals beyond the system boundary, resulting from 2021.
the treatment of recycled materials from the point of end-of-
3.8 Geographic Representativeness
waste to the point of substitution (as loads) and substitution of
primary resources (as benefits). Land or region, in which the declared product system is
It also includes the benefits and burdens associated with manufactured, used or handled at the end of the product´s
energy recovery from plastic waste in a municipal waste lifespan: Europe
incineration plant, as modelled in Module C3.
In Module D, only net flows of metals leaving the product
3.9 Allocation
system are considered.
No co-products are generated during the production of the
3.3 Estimates and assumptions VELUX products. Sorted production scrap of the different
metals, notably aluminium, is considered a secondary material
No further assumptions and estimates relevant to the result had
with no economic value (so no burdens allocated) and
to be made beyond the points made in this chapter 3 and
considered in the quantification of net flows leaving the product
chapter 4.
system. This approach is chosen to ensure a coherent
3.4 Cut-off criteria quantification of net flows entering module D.
No data available from the company survey was neglected.
These include, among other things, material use, energy No processes were modelled as part of the foreground model
demand (heat, electricity), packaging materials of raw materials that would have required an allocation of multi-input processes.
(in so far as they are generated as waste) and product Background datasets on municipal waste incineration plants
packaging, consumables in production, waste treatment and were taken from ecoinvent v3.8 (cut-off) without any
the transport of all inputs and outputs. modification.
With this approach, mass and energy flows below 1% were also
accounted for, up to a total of 5%. No processes were Allocation of reuse, recycling and recovery was avoided by the
neglected that would have been known to the project managers cut-off approach in the foreground model in line with DIN EN
and would have contributed significantly to the indicators of the 15804.
impact assessment.
3.10 Comparability
3.5 Background data Basically, a comparison or an evaluation of EPD data is only
Ecoinvent v3.8 (cut-off) (2021) is used as the background possible if all the data sets to be compared were created
database. according to EN 15804 and the building context, respectively
the product-specific characteristics of performance, are taken
3.6 Data quality into account.
The foreground data are based on extensive and detailed data Ecoinvent v3.8 (cut-off) has been used as the background
collection at the production site. The foreground data could be database.
4. LCA: Scenarios and additional technical information
quantification, an efficiency of 25.6% is assumed for the
Characteristic product properties of biogenic carbon production of heat and 13.0% for the production of electricity
Information on describing the biogenic carbon content at (always referring to the lower heating value of the waste).
factory gate Metals and cardboard are recycled; it is assumed that these
fractions reach the end-of-waste state after having been sorted
Name ValueUnit
and transported (as a conservative choice) to a recycler over
kg
Biogenic carbon content in product - 150 km with a lorry with a payload of 16-32 metric tons,
C
EURO6.
Biogenic carbon content in accompanying kg No packaging waste is landfilled.
< 5%
packaging C The use of multi-way pallets is not taken into account as
packaging material.
Note: 1 kg of biogenic carbon is equivalent to 44/12 kg of CO .
2
Module A5
The products are delivered to the construction site ready to be
installed. Manual installation is assumed, and electricity
consumption related to electric drilling machines, screwdrivers,
etc. is considered to be negligible.
The combustible packaging material (plastics) is assumed to be
transported 50 km with a lorry with a payload of 16-32 metric
tons, EURO6 to an incineration plant with an efficiency R1 < 0.6
(according to the ecoinvent v3.8 (cut-off) dataset used); the
recovered energy is declared as exported energy; for its
4 Environmental Product Declaration - VELUX A/S - VELUX sun tunnel TCF for flat roof, flexible, acrylic dome
Module C1
Reference service life Manual de-installation is assumed, electricity consumption
Name Value Unit related to electric screw drivers, etc. is considered to be
negligible. Thus, no environmental impacts are declared in
Reference service life
module C1.
according to 30 a
manufacturer's declaration
Module C2
The product has passed
Declared product Given the complexity of the inventoried products, a mixed end-
internal quality controls and
properties (at the gate) and - of-life scenario is modelled, allowing the different materials to
complies with EN 1873 for CE
finishes follow their most likely path.
marking
It should also be noted that the deconstruction and waste
The product has passed treatment scenario can vary a lot, depending on the actual
Declared product
internal quality controls and situation. Thus, a generic end-of-life scenario is assumed.
properties (at the gate) and -
complies with EN 1873 for CE As a rule of thumb, metals are recycled, plastics are incinerated
finishes
marking (also due to the very limited availability on plastics recycling
An assumed quality of and its benefits).
Carried out in accordance
work, when installed in The combustible material (mainly plastics) is assumed to be
with the manufacturer's -
accordance with the transported 50 km with a lorry with a payload of 16-32 metric
instructions.
manufacturer’s instructions tons, EURO6 to an incineration plant.
Design application Metals are recycled; it is assumed that these fractions reach the
parameters (if instructed by end-of-waste state after having been sorted and transported to
the manufacturer), Installation according to a recycler over 150 km with a lorry with a payload of 16-32
including the references to assembly instructions and - metric tons, EURO6.
state of the art.
the appropriate practices
and application codes Module C3
A consumption of 0.03 kWh/kg of electricity for shredding and
Outdoor environment, (for The declared products are
sorting and 0.437 MJ/kg of diesel fuel for internal logistics are
outdoor applications), e.g. intended for installation
taken into account to disassemble the product. The recovered
weathering, pollutants, UV outside the building: They are
- material leaves the product system as 'materials for recycling'.
and wind exposure, therefore designed to
The net amounts of the metals leaving the product system are
building orientation, withstand outdoor conditions
considered as 'use of secondary material' in Module D.
shading, temperature throughout their service life.
Indoor environment (for
The declared products are Module C4
indoor applications), e.g.
not intended for installation - As stated above, it is assumed that 100% of the plastic parts
temperature, moisture,
inside a building. are treated in a waste incineration plant with an efficiency R1
chemical exposure
< 0.6 (according to the ecoinvent v3.8 (cut-off) dataset used);
Indoor environment (for The declared products are 25.57% of the lower heating value of the plastic parts are
indoor applications), e.g. not intended for installation - recovered as heat and 13.0% as electricity. Recovered energy
temperature, moisture, inside a building. is reported as 'exported energy' and considered in Module D.
chemical exposure
Usage conditions, e.g. Standard use in any type of Module D
frequency of use, building, i.e. opening/closing - Module D contains the benefits and loads beyond the system
mechanical exposure as often as necessary. boundary related to the recycling of metals, which result from
The declared products are the treatment of recycled materials from the point of end-of-
Maintenance e.g. required designed for a reference life waste status to the point of substitution (as loads) and the
frequency, type and quality of 30 years. They are substitution of primary resources (as benefits).
-
and replacement of maintained by cleaning water Due to a lack of data for plastics from de-construction activities,
components at the discretion of the the substitution potential of recycled plastics is not taken into
building occupants. account.
Only net flows leaving the product system are considered in
module D.
5 Environmental Product Declaration - VELUX A/S - VELUX sun tunnel TCF for flat roof, flexible, acrylic dome
5. LCA: Results
DESCRIPTION OF THE SYSTEM BOUNDARY (X = INCLUDED IN LCA; MND = MODULE OR INDICATOR NOT DECLARED; MNR
= MODULE NOT RELEVANT)
Benefits and
Construction loads beyond
Product stage Use stage End of life stage
process stage the system
boundaries
la ire ta m w a Ry lp p u s tro p s n a rT g n iru tc a fu n a M e h t m o rf tro p s n a rTe tis e h t o t e ta g y lb m e s s A e s U e c n a n e tn ia M ria p e R tn e m e c a lp e R tn e m h s ib ru fe R y g re n e la n o ita re p Oe s u re ta w la n o ita re p Oe s u n o itc u rts n o c -e Dn o itilo m e d tro p s n a rT g n is s e c o rp e ts a W la s o p s iD -e s u e R-y re v o c e R-g n ilc y c e Rla itn e to p
A1 A2 A3 A4 A5 B1 B2 B3 B4 B5 B6 B7 C1 C2 C3 C4 D
X X X MND X MND MND MNR MNR MNR MND MND X X X X X
RESULTS OF THE LCA - ENVIRONMENTAL IMPACT according to EN 15804+A2: 1 piece VELUX sun tunnel TCF 0K14 0010 for
flat roof, flexible, acrylic dome
Parameter Unit A1-A3 A5 C1 C2 C3 C4 D
GWP-total kg CO 2 eq 4.56E+01 2.73E+00 0 7.33E-02 2.63E-01 2.06E+01 -1.24E+01
GWP-fossil kg CO 2 eq 4.76E+01 7.66E-01 0 7.32E-02 2.04E-01 2.05E+01 -1.24E+01
GWP-biogenic kg CO 2 eq -2.03E+00 1.97E+00 0 0 5.91E-02 0 0
GWP-luluc kg CO 2 eq 6.19E-02 2.43E-05 0 2.98E-05 2.27E-04 5.33E-03 -1.66E-02
ODP kg CFC11 eq 1.02E-05 1.37E-08 0 1.72E-08 1.26E-08 1.81E-06 -8.53E-07
AP mol H+ eq 2.06E-01 3.99E-04 0 4.15E-04 7.8E-04 2.08E-02 -3.59E-02
EP-freshwater kg P eq 1.36E-03 4.76E-07 0 5.39E-07 2.65E-05 1.58E-04 -9.07E-04
EP-marine kg N eq 3.92E-02 1.52E-04 0 1.49E-04 2.5E-04 4.82E-03 -6.13E-03
EP-terrestrial mol N eq 4.06E-01 1.68E-03 0 1.64E-03 2.84E-03 5.3E-02 -7.07E-02
kg NMVOC
POCP 1.39E-01 4.71E-04 0 4.7E-04 7.57E-04 1.41E-02 -2.11E-02
eq
ADPE kg Sb eq 5.78E-04 2.03E-07 0 2.45E-07 3.56E-07 4.22E-05 -4.29E-05
ADPF MJ 8.17E+02 8.98E-01 0 1.13E+00 2.82E+00 4.03E+01 -1.69E+02
m3 world eq
WDP 2.19E+01 3.9E-03 0 3.7E-03 7.02E-03 3.01E+00 -8.21E-01
deprived
GWP = Global warming potential; ODP = Depletion potential of the stratospheric ozone layer; AP = Acidification potential of land and water; EP =
Eutrophication potential; POCP = Formation potential of tropospheric ozone photochemical oxidants; ADPE = Abiotic depletion potential for non-fossil
resources; ADPF = Abiotic depletion potential for fossil resources; WDP = Water (user) deprivation potential)
RESULTS OF THE LCA - INDICATORS TO DESCRIBE RESOURCE USE according to EN 15804+A2: 1 piece VELUX sun tunnel
TCF 0K14 0010 for flat roof, flexible, acrylic dome
Parameter Unit A1-A3 A5 C1 C2 C3 C4 D
PERE MJ 2.3E+01 2.26E+01 0 1.59E-02 3.56E-01 4.56E+00 -1.59E+01
PERM MJ 2.34E+01 -2.26E+01 0 0 -7.61E-01 0 0
PERT MJ 4.64E+01 1.41E-02 0 1.59E-02 -4.05E-01 4.56E+00 -1.59E+01
PENRE MJ 5.79E+02 1.03E+01 0 1.13E+00 2.25E-06 2.69E+02 -1.7E+02
PENRM MJ 2.38E+02 -9.37E+00 0 0 0 -2.28E+02 0
PENRT MJ 8.17E+02 8.98E-01 0 1.13E+00 2.25E-06 4.04E+01 -1.7E+02
SM kg 4.49E-01 0 0 0 0 0 1.37E+00
RSF MJ 0 0 0 0 0 0 0
NRSF MJ 0 0 0 0 0 0 0
FW m3 5.08E-01 2.13E-04 0 1.23E-04 6.73E-04 7.98E-02 -4.13E-02
PERE = Use of renewable primary energy excluding renewable primary energy resources used as raw materials; PERM = Use of renewable primary
energy resources used as raw materials; PERT = Total use of renewable primary energy resources; PENRE = Use of non-renewable primary energy
excluding non-renewable primary energy resources used as raw materials; PENRM = Use of non-renewable primary energy resources used as raw
materials; PENRT = Total use of non-renewable primary energy resources; SM = Use of secondary material; RSF = Use of renewable secondary fuels;
NRSF = Use of non-renewable secondary fuels; FW = Use of net fresh water
RESULTS OF THE LCA – WASTE CATEGORIES AND OUTPUT FLOWS according to EN 15804+A2:
1 piece VELUX sun tunnel TCF 0K14 0010 for flat roof, flexible, acrylic dome
Parameter Unit A1-A3 A5 C1 C2 C3 C4 D
HWD kg 1.9E-03 2.45E-06 0 2.87E-06 2.25E-06 7.1E-05 6.22E-05
NHWD kg 9.63E+00 6.88E-02 0 7.55E-02 1.15E-02 1.14E+00 -2.26E+00
RWD kg 2.36E-03 1.27E-05 0 1.63E-05 2.55E-05 3E-04 -6.97E-04
CRU kg 0 0 0 0 0 0 0
MFR kg 1.12E+00 1.35E+00 0 0 8.01E-01 0 0
MER kg 0 0 0 0 0 0 0
EEE MJ 4.31E-01 1.22E+00 0 0 0 2.97E+01 0
6 Environmental Product Declaration - VELUX A/S - VELUX sun tunnel TCF for flat roof, flexible, acrylic dome
EET MJ 8.48E-01 2.39E+00 0 0 0 5.83E+01 0
HWD = Hazardous waste disposed; NHWD = Non-hazardous waste disposed; RWD = Radioactive waste disposed; CRU = Components for re-use;
MFR = Materials for recycling; MER = Materials for energy recovery; EEE = Exported electrical energy; EET = Exported thermal energy
RESULTS OF THE LCA – additional impact categories according to EN 15804+A2-optional:
1 piece VELUX sun tunnel TCF 0K14 0010 for flat roof, flexible, acrylic dome
Parameter Unit A1-A3 A5 C1 C2 C3 C4 D
Disease
PM 2.71E-06 6.84E-09 0 8.09E-09 1.23E-08 1.65E-07 -3.43E-07
incidence
IR kBq U235 eq 1.26E+00 3.85E-03 0 4.89E-03 9.79E-03 1.74E-01 -2.92E-01
ETP-fw CTUe 1E+03 3.36E+00 0 8.93E-01 1.66E+00 7.61E+02 -1.38E+02
HTP-c CTUh 8.54E-08 1.27E-10 0 3.56E-11 4.48E-11 5.81E-09 -1.94E-08
HTP-nc CTUh 7.16E-07 1.63E-09 0 1.03E-09 1.46E-09 1.98E-07 -1.11E-07
SQP SQP 1.78E+02 7.53E-01 0 9.62E-01 3.81E-01 1.17E+01 -1.9E+01
PM = Potential incidence of disease due to PM emissions; IR = Potential Human exposure efficiency relative to U235; ETP-fw = Potential comparative
Toxic Unit for ecosystems; HTP-c = Potential comparative Toxic Unit for humans (cancerogenic); HTP-nc = Potential comparative Toxic Unit for humans
(not cancerogenic); SQP = Potential soil quality index
Disclaimer 1 – for the indicator “Potential Human exposure efficiency relative to U235”.This impact category deals mainly with the
eventual impact of low dose ionizing radiation on human health of the nuclear fuel cycle. It does not consider effects due to possible
nuclear accidents, occupational exposure or radioactive waste disposal in underground facilities. Potential ionizing radiation from the
soil, radon and from some construction materials is also not measured by this indicator.
Disclaimer 2 – for the indicators “abiotic depletion potential for non-fossil resources”, “abiotic depletion potential for fossil resources”,
“water (user) deprivation potential, deprivation-weighted water consumption”, “potential comparative toxic unit for ecosystems”,
“potential comparative toxic unit for humans – cancerogenic”, “Potential comparative toxic unit for humans - not cancerogenic”,
“potential soil quality index”. The results of this environmental impact indicator shall be used with care as the uncertainties on these
results are high as there is limited experience with the indicator.
6. LCA: Interpretation
Figure 1 illustrates the relative contributions of the different A1-A3 = 100%).
modules along the life cycle of the declared products (Modules
significance depending on the indicator and fluctuate between -
Figure 1: Relative environmental impacts of the different 5% and -60%.
life cycle stages for the VELUX sun tunnel TCF 0K14 0010 The use of renewable primary energy is mainly caused by the
(Modules A1-A3 = 100%) share of renewable energy in the electricity mix, thus the
production stage is the main driver of this impact category; the
The LCA is dominated by the manufacture of the product same holds also for the use of non-renewable primary energy.
(modules A1-A3); further relevant contributions come only from Material use of primary energy is negligible and related to
the incineration of the plastic waste in module C4. plastic parts of the product and packaging material. The
The benefits and burdens outside the product system vary in material use of primary energy is transferred to its energy use
7 Environmental Product Declaration - VELUX A/S - VELUX sun tunnel TCF for flat roof, flexible, acrylic dome
when the materials containing primary energy are incinerated ores and related to the disposal of road infrastructure;
with energy recovery. hazardous and radioactive waste are mainly caused by the
Non-hazardous waste as the quantitatively most relevant waste nuclear power in the electricity mix.
flows is mainly caused during mining andprocessing of metal
7. Requisite evidence
7.1 Formaldehyde standard.
Not tested based on applicable product standard.
7.2 MDI 7.4. Fire gas toxicity
Not tested based on applicable product standard. Not tested based on applicable product standard.
7.3 Checking of pre-treatment of substances used
according to AltholzVO 7.5 VOC emissions
Not applicable; not tested based on applicable product Not tested based on applicable product standard.
8. References
Product category rules of IBU ISO 14001
DIN EN ISO 14001:2015: Environmental management
IBU (2021) systems - Requirements with guidance for use.
IBU (2021): General Instructions for the EPD Programme of the
Institut Bauen und Umwelt e.V.. Version 2.0, Institut Bauen und ISO 45001
Umwelt e.V., Berlin ISO 45001:2018-03, Occupational health and safety
management systems - Requirements with guidance for use.
IBU (2022)
IBU (2022): Product category rules for building-related products EN 1873
and service, PCR Part A: Calculation rules for the life cycle DIN EN 1873:2005, Prefabricated accessories for roofing -
assessment and requirements for the project report. Version Individual rooflights of plastics - product specification and test
2.2., Institut Bauen und Umwelt e.V., Berlin. methods.
IBU (2023) ECHA candidate list
IBU (2023): PCR Guidance-Texts for Building-Related Products The Candidate List of Substances of Very High Concern for
and Services, PCR Part B: Requirements on the EPD for Authorisation, European Chemicals Agency, Helsinki.
windows and doors. Version 2023/04, Institut Bauen und
Umwelt e.V., Berlin. Regulation on biocidal products
REGULATION (EU) No 528/2012 OF THE EUROPEAN
Standards and legal documents PARLIAMENT AND OF THE COUNCIL of 22 May 2012
concerning the making available on the market and use of
EN 15804 biocidal products.
DIN EN 15804+A2:2022-3, Sustainability of construction
works - Environmental product declarations - Core rules for the Regulation (EU) Nr. 305/2011(CPR)
product category construction products. German version EN REGULATION (EU) No 305/2011 OF THE EUROPEAN
15804:2012+A2:2019 + AC:2021 PARLIAMENT AND OF THE COUNCIL of 9 March 2011 laying
down harmonised conditions for the marketing of construction
ISO 14025 products and repealing Council Directive 89/106/EEC.
DIN EN ISO 14025:2006-07, Environmental labels and
declarations - Type III Environmental declarations - Principles COUNCIL REGULATION (EU) No 333/2011
and procedures. COUNCIL REGULATION (EU) No 333/2011 of 31 March 2011
establishing criteria determining when certain types of scrap
ISO 14044 metal cease to be waste under Directive 2008/98/EC of the
DIN EN ISO 14044:2006-07, Environmental management - Life European Parliament and of the Council.
cycle assessment - Requirements and guidance (ISO
14044:2006); German and English versions EN ISO European Waste List (Waste index)
14044:2006. http://www.gesetze-im-internet.de/avv/anlage.htm
ISO 9001 Additional references
DIN EN ISO 9001:2015, Quality management systems -
Requirements. ecoinvent 3.8
ecoinvent 3.8, LCA database, 12/2021. Ecoinvent centre,
Zürich.
8 Environmental Product Declaration - VELUX A/S - VELUX sun tunnel TCF for flat roof, flexible, acrylic dome
Publisher
Institut Bauen und Umwelt e.V. +49 (0)30 3087748- 0
Hegelplatz 1 info@ibu-epd.com
10117 Berlin www.ibu-epd.com
Germany
Programme holder
Institut Bauen und Umwelt e.V. +49 (0)30 3087748- 0
Hegelplatz 1 info@ibu-epd.com
10117 Berlin www.ibu-epd.com
Germany
Author of the Life Cycle Assessment
Dr. Frank Werner - Umwelt & Entwicklung + 41 (0)44 241 39 06
Kammelenbergstrasse 30 frank@frankwerner.ch
9011 St. Gallen http://www.frankwerner.ch/
Switzerland
Owner of the Declaration
VELUX Group +4545164726
Ådalsvej 99 jakob.roerbech@velux.com
2970 Hørsholm www.velux.com
Denmark
9 Environmental Product Declaration - VELUX A/S - VELUX sun tunnel TCF for flat roof, flexible, acrylic dome
