ENVIRONMENTAL PRODUCT DECLARATION
as per ISO 14025 and EN 15804+A1
Owner of the Declaration Troldtekt A/S
Programme holder Institut Bauen und Umwelt e.V. (IBU)
Publisher Institut Bauen und Umwelt e.V. (IBU)
Declaration number EPD-TRO-20210109-ICA1-EN
Issue date 27.04.2021
Valid to 26.04.2026
Acoustic panels - painted
Troldtekt 25 mm Natural Wood
www.ibu-epd.com | https://epd-online.com
Umwelt Produktdeklaration Name des Herstellers – Name des Produkts
1. General Information
Troldtekt A/S Natural Wood, painted
Programme holder Owner of the declaration
IBU – Institut Bauen und Umwelt e.V. Troldtekt A/S
Panoramastr. 1 Sletvej 2 A
10178 Berlin 8310 Tranbjerg
Germany Denmark
Declaration number Declared product / declared unit
EPD-TRO-20210109-ICA1-EN Acoustic panel "Natural Wood" - 1m2, 25 mm thickness
- painted finish
This declaration is based on the product Scope:
category rules: This declaration represents the production, supply,
Wood cement - Mineral-bonded wooden composites, mounting, use, dismantling and disposal of 1 m2 (25
01.2019 mm thickness) of white cement-bonded wood wool
(PCR checked and approved by the SVR) acoustic panel "Natural Wood" with a painted
finish, produced by Troldtekt A/S, with a reference
service life of 50 years. The production facility is
Issue date
located in Jutland, Denmark. Three scenarios
27.04.2021
represent its use in indoor conditions in Denmark,
Sweden and Germany.
Valid to
26.04.2026
The owner of the declaration shall be liable for the
underlying information and evidence; the IBU shall not
be liable with respect to manufacturer information, life
cycle assessment data and evidences.
The EPD was created according to the specifications
of EN 15804+A1. In the following, the standard will be
simplified as EN 15804.
Verification
The standard EN 15804 serves as the core PCR
Independent verification of the declaration and data
according to ISO 14025:2010
Dipl. Ing. Hans Peters internally x externally
(chairman of Institut Bauen und Umwelt e.V.)
Dr. Alexander Röder Ms Jane Anderson
(Managing Director Institut Bauen und Umwelt e.V.)) (Independent verifier)
2. Product
2.1 Product description/Product definition 2.2 Application
Troldtekt Natural Wood acoustic panels are some of The panels are installed on the ceilings and walls in
the leading and preferred solutions for creating a good offices, businesses, schools, institutions, cultural sites,
indoor sound environment. They are sold in sports centers, swimming pools and private homes.
various thicknesses (20-35 mm) and dimensions
(width: 600 mm, lengths: 600/1200/2400 mm or width: 2.3 Technical Data
625 mm, lengths: 625/1250/2500 mm). The panels can The table below indicates the technical specifications
be unpainted or painted in a wide variety of colors. of the panels in accordance with EN 13168, the
standard for cement-bonded wood wool and double-
For the placing on the market of the product in the layer panels with cement-bonded wood wool, and EN
European Union/European Free Trade Association 13964, the standard for suspended ceilings.
(EU/EFTA) (with the exception of Switzerland)
Regulation (EU) No. 305/2011 (CPR) applies. The
product needs a declaration of performance taking into
consideration EN 13964:2014, Suspended ceilings.
Requirements and test methods, and the CE-marking.
For the application and use, the respective national
provisions apply.
2 Environmental Product Declaration Troldtekt A/S – Troldtekt 25mm Natural Wood - painted
Technical specifications of the product covered in
this EPD 2.9 Packaging
Name Value Unit The product is packaged with plastic film and
Gross density 469 kg/m3 cardboard. The packaging material can be easily
Grammage 11,73 kg/m2 sorted and treated in dedicated waste recycling
Thermal conductivity acc. to DIN channels. The packaged product is delivered on a
76 W/(mK)
52612 returnable wood pallet.
Water vapour diffusion resistance
- -
factor acc. to DIN 4108-4
Sound absorption coefficient (only with 2.10 Condition of use
reference to the corresponding - % Conditions of use are detailed
component design) here: https://www.troldtekt.com/Installation/Use_and_
Light reflection (measured by DELTA 26,3 - maintenance
%
Light and Optics 70,8
Reaction to fire B/S1/d0 2.11 Environment and health during use
Environmental and ecotoxicity risks from exposure to
Troldtekt panel products during use have been
assessed and found eligible to the following
Performance data of the product in accordance with
certification schemes:
the declaration of performance with respect to its
essential characteristics according to EN  Finnish M1 classification
13168:2012+A1:2015, Thermal insulation products for  Danish Indoor Climate
buildings. Factory made wood wool (WW) products.
Specification, and EN 13964:2014, Suspended
These certificates can be accessed
ceilings. Requirements and test methods.
here: https://www.troldtekt.com/Web-
tools/Downloads/Certificates-and-tests
2.4 Delivery status
The panel is usually distributed in length of 600,
2.12 Reference service life
1200 or 2400 mm by 600 mm width or in length of 625,
The technical service life of the panel is superior to 50
1250 or 2500 mm by 625 mm width. It comes in
years. This EPD refers to the service lifetime indicated
three thicknesses: 20, 25 and 35 mm. Additionally,
by the BBSR table for the material 353.311 of type
several density ranges are available: Coarse, Fine,
“Holzbekleidungen: Holz, Holzwerkstoff und
Ultra-Fine and Extreme-Fine causing different
Mehrschichtleichtbauplatten”.
densities (388-428 kg/m3). The panels are normally
delivered in packs of 80 units on pallets.
Because the panel is used in a building, in this EPD its
reference service life is limited by the expected service
2.5 Base materials/Ancillary materials
life of the building, which is commonly accepted as 50
The composition of the finished product is a mix of
years, at least as LCA timeframe.
wood wool (31,3%), Portland cement (58,3%), water
(7,8%), as well as water glass (<1%) and accelerator
There is no influence of the ageing of the material on
(<1%). Additionally, a painted finish is provided with a
its technical performances.
water-based paint (1,2%). The composition is at dry
basis at the factory gate, as most of the water has
2.13 Extraordinary effects
evaporated during drying, but water remains bound to
the wood fibre and cement paste (hydrated cement).
Fire
Information on the fire performance according to EN
2.6 Manufacture
13168.
Norway spruce logs from local forests (with a moisture
content of about 65-70%) are received and the bark is
Fire protection
removed. The wood is stored for approximately six
Name Value
months until the moisture content in the wood drops to
Building material class B
29%. The wood is then shredded to produce wool. The
Burning droplets d0
wood wool is mixed together with Portland cement,
Smoke gas development S1
water, and additives. The mixture is cast and cured
using a heat press and dried with a biomass-fired
Water
oven. The cast panel is milled to remove any material
No information on the product performance under the
in excess and cut edges. After approximately 4 weeks
unforseeable influence of water is available.
of curing, the panel can be painted before being stored
on a pallet and packaged to be transported to central
Mechanical destruction
distribution warehouses.
No information on the product performance under
unforseeable mechanical destruction is available.
2.7 Environment and health during
manufacturing
2.14 Re-use phase
Troldtekt is following its working environment closely.
Currently, Troldtekt panels undergo thermal treatment
Both the physical working environment and sickness
with energy recovery. Composting is also possible.
absence are closely monitored. It is an ongoing
process involving both leaders and factory workers.
Additional information on recycling
options: https://www.troldtekt.com/~/media/Files/Info%
2.8 Product processing/Installation
20sheets/English/Troldtekt_Recycling%20instructions
Installation instructions are available here:
%20pdf.pdf
https://www.troldtekt.com/Installation
3 Environmental Product Declaration Troldtekt A/S – Troldtekt 25mm Natural Wood - painted
2.15 Disposal Additional information on disposal
The product may be composted, thermally treated with options: https://www.troldtekt.com/environment-and-
energy recovery, or landfilled. csr/product-life-cycle/recycling/
European Waste Code: 10 13 11 (wastes from 2.16 Further information
cement-based composite materials) For additional information on technical specifications,
you may consult the Declaration Of
Painted panels must be incinerated at end-of-life. Performance: https://www.troldtekt.com/Web-
tools/Downloads/DoPs
3. LCA: Calculation rules
3.1 Declared Unit samples used to build inventories are based on the
The functional unit is 1 m2 of acoustic panel, in 25 mm entirety of the annual production of panels in 2020 and
thickness, corresponding to 11,73 kg of material with a is verified by a third party. Such representativeness is
painted finish, mounted on ceiling, with a reference also valid for the production of Portland cement, whose
service life of 50 years. EPDs, however, were published in 2021 (white) and
2017 (grey). The EPD for the paint used was published
Declared unit in 2018.
Name Value Unit
Declared unit 1 m2 Temporal, geographical and technological
Gross density 469 kg/m3 representativeness
Grammage 11.73 kg/m2 All data strictly related to the cement production is
conversion factor [Mass/Declared technologically, temporally, and geographically
11.73 -
Unit] representative. The cement production data is less
Layer thickness 0.025 m than 5 years old. However, since the improvement in
grey cement production processes in the meantime
have not been accounted for, the LCA results for the
Troldtekt panels based on grey cement can be said to
3.2 System boundary be conservative. The data used to model the
Cradle to grave foreground inventory of acoustic panels dates from the
production year of 2020. As for secondary data, some
3.3 Estimates and assumptions most of the ecoinvent datasets are less than 3 years
Assumptions are described occasionally throughout old.
the section "LCA: Calculation rules".
3.7 Period under review
3.4 Cut-off criteria The primary data concerned with the manufacture (A1-
The cut-off criterion is applied according to EN A3) relates to the production year 2020 and the data
15804 Section 6.3.5 and PCR part A Section 5.6. are based on the volumes produced on an annual
All inputs and outputs for which data are available are basis.
included in the LCA model. Data gaps are filled with
conservative assumptions from average data (when 3.8 Allocation
available) or with generic data and are documented Allocation of production data to the multiple produced
accordingly. types of panels (with the same functional unit) is
The following product flows have been omitted performed based on the rules provided in EN 15804.
according to the 1% cut-off rule: Sub-processes associated to painting have specially
 Wooden pallet to transport the product been allocated to the painted panels. Data such as
waste generation and packaging have been allocated
 Capital infrastructure (factory)
to the entire production volume of panels in Troldtekt.
 Energy utilization of incinerated paint
The only case of co-produced outputs is associated to
 Allocation of burden from wood logging to wood logging. However, the environmental load is
residual wood fractions evenly distributed over all its co-products, such as
logs, energy wood, and bark.
3.9 Comparability
3.5 Background data
Basically, a comparison or an evaluation of EPD data
Two types of data source are used as secondary data:
is only possible if all the data sets to be compared
 Product-specific EPDs for the manufacture
were created according to EN 15804 and the building
and supply of Portland cement and water- context, respectively the product-specific
based paint characteristics of performance, are taken into account.
 Database ecoinvent v.3.6 cut-off
The used background database is ecoinvent v.3.6 cut-
off
3.6 Data quality
Statistical representativeness
The statistical representativeness of the product
system is very good. The input and output data
4. LCA: Scenarios and additional technical information
4 Environmental Product Declaration Troldtekt A/S – Troldtekt 25mm Natural Wood - painted
Manufacture (A1-A3) Electricity consumption 0,060 kWh
Material loss (plastic film) 0,007 kg
Data Material loss (cardborad) 0,032 kg
Primary data is third-party verified and based on the Use phase (B1)
production year 2020, within the facilities of Troldtekt Prior to distribution and during the use phase (B1), the
A/S in Jutland (Denmark). carbonation of the cement contained in the panel,
during use, is accounted for. Based on laboratory
End-of-waste state and use of by-products measurement, the panel will absorb up to 140 grams of
For all processes supplying a residual material/waste carbon dioxide per kilogram of cement. Normalized to
that originates the end-of-life phase of a product to the the reference flow, this corresponds to an uptake of
product system to be used as input, the polluter-pay approximately 0,9 kilograms of carbon dioxide by the
principle “100:0” is used. Some wooden by-products end of the service lifetime, including the uptake in A3.
generated during manufacture in Troldtekt end up as
soil improvers externally (reaching end-of-waste state), Maintenance (B2)
and thus their biogenic carbon leaves Troldtekt's As the panel does not require any maintenance except
system boundary. for the occasional dusting, no maintenance module
(B2) is considered.
Wind-certified electricity
All the electricity used to produce the panels in the Information about reference service life is detailed in
Module A3 originates from Danish wind power, for 2.12.
which a certificate ensures the origin. It originates from
a 1-3 MW offshore wind turbine, with transformation, Reference service life
transmission and distribution losses and is modelled Name Value Unit
correspondingly. Reference service life (according to
50 a
ISO 15686-1, -2, -7 and -8)
Carbon balance Life Span (according to BBSR) 50 a
Biogenic: Absorption of biogenic CO 2 by the purchased Life Span according to the
wood has been considered in A1. Some of it is manufacturer 75 a
released again during production in A3, some ends up
sequestered in soil, while the majority of the remaining
End of life (C1-C4)
biogenic CO , 7,02 kg, is retained in the finished
2 Name Value Unit
product and emitted during end-of-life incineration in
Electricity use (for un-mounting) 0,060 kWh
C4.
Transport (to material sorting facility) 50 km
Fossil: Absorption of some fossil CO , originating from
2 Collected as mixed construction waste 11,73 kg
the calcination of limestone during cement production,
Energy recovery 3,58 kg
happens when the cement is mixed with water in A3. A
Energy recovery efficiency 10 %
majority is absorbed during the use phase B1, and all
Energy recovered 7,30 MJ
the absorbed fossil CO is finally emitted during end-
2
of-life incineration in C4.
The panel is un-mounted at the end of its reference
service life and driven to the regional waste
Distribution to site (A4) and mounting (A5)
incineration plant. Energy is recovered from the wood
To consider the main geographical variants of the life
part of the panel at 10% efficiency.
cycle of Troldtekt Natural Wood panels, three
scenarios are developed, where the product is
supplied, mounted, used and discarded in Aarhus
(Denmark), Hamburg (Germany) and Malmö Reuse, recovery and/or recycling potentials (D),
(Sweden). An additional 50 km from the local relevant scenario information
warehouse to construction site is assumed. Name Value Unit
Electricity 1,73 MJ
Heat 5,57 MJ
Transport to the building site (A4)
Name Value Unit The energy substituted from incineration of the panel's
Litres of fuel 26,8 l/100km wood component in C4 is considered being a split of
Transport distance to Denmark 160 km the Danish electricity grid mix (for electricity) and
Transport distance to Germany 370 km natural gas (for heat).
Transport distance to Sweden 394 km
Transport distance from Details on possible disposal routes
warehouse to local construction Aalborg Portland cement factory utilizes dust and
50 km
sites in offcuts from the Troldtekt factory as a raw material in
Denmark/Germany/Sweden new cement, i.e. in the technical circle. During
Capacity utilisation (including incineration in the cement kiln, the wood content in the
85 %
empty runs) cement bonded wood wool panels replaces fossil fuels,
Gross density of products while the cement ends up as a raw material in new
transported 405 kg/m3 cement, replacing virgin raw materials and heavy fossil
Capacity utilisation volume factor 1 - fuels, thereby avoiding a significant amount of CO 2
emissions. This scheme of wood wool waste as a raw
material can be scaled for construction site and
demolition waste. It will be gradually rolled out to all of
Denmark in the period 2021-2023. Once Denmark has
Installation into the building (A5)
documented economic and environmental benefits to
Name Value Unit
be gained by including wood wool waste in the
5 Environmental Product Declaration Troldtekt A/S – Troldtekt 25mm Natural Wood - painted
production of new cement rather than going to waste
incineration or landfill, dialogue with municipalities and
local cement producers in the primary markets of
Troldtekt is initiated to facilitate similar schemes
regionally or nationally.
6 Environmental Product Declaration Troldtekt A/S – Troldtekt 25mm Natural Wood - painted
5. LCA: Results
Note: Global Warming Potential (GWP) indicator includes CO of both biogenic and fossil origin.
2
Also, GWP results for Troldtekt Natural Wood (painted) for other delivery scenarios in respectively Germany and
Sweden, are 2,30E-1 kg CO and 2,43E-1 kg CO .
2 2
DESCRIPTION OF THE SYSTEM BOUNDARY (X = INCLUDED IN LCA; MND = MODULE NOT DECLARED;
MNR = MODULE NOT RELEVANT)
BENEFITS AND
CONSTRUCTI LOADS
PRODUCT STAGE ON PROCESS USE STAGE END OF LIFE STAGE BEYOND THE
STAGE SYSTEM
BOUNDARIES
7 Environmental Product Declaration Troldtekt A/S – Troldtekt 25mm Natural Wood - painted
lairetam
waR
ylppus tropsnarT
gnirutcafunaM
eht
morf
tropsnarT
etis
eht
ot
etag
ylbmessA esU
ecnanetniaM
riapeR
tnemecalpeR tnemhsibrufeR
ygrene
lanoitarepO esu
retaw
lanoitarepO esu
noitcurtsnoc-eD
noitilomed tropsnarT
gnissecorp
etsaW
lasopsiD -esueR -yrevoceR -gnilcyceR laitnetop
A1 A2 A3 A4 A5 B1 B2 B3 B4 B5 B6 B7 C1 C2 C3 C4 D
X X X X X X MND MNR MNR MNR MND MND X X MND X X
RESULTS OF THE LCA - ENVIRONMENTAL IMPACT according to EN 15804+A1: 1 m2 Natural Wood, 25
mm, painted finish, delivered and used in Denmark
Parameter Unit A1-A3 A4 A5 B1 C1 C2 C4 D
GWP [kg CO2-Eq.] 1.73E+0 1.15E-1 8.57E-2 -7.34E-1 6.50E-4 9.69E-2 7.99E+0 -5.54E-1
ODP [kg CFC11-Eq.] 3.34E-7 2.09E-8 1.64E-9 0.00E+0 2.81E-10 1.77E-8 6.41E-9 -3.84E-8
AP [kg SO2-Eq.] 4.48E-2 2.32E-4 5.90E-5 0.00E+0 1.59E-6 1.96E-4 5.30E-4 -8.01E-4
EP [kg (PO4)3--Eq.] 1.02E-2 4.77E-5 1.03E-4 0.00E+0 8.86E-7 4.03E-5 2.30E-4 -4.64E-4
POCP [kg ethene-Eq.] 2.77E-3 1.53E-5 2.58E-6 0.00E+0 8.88E-8 1.29E-5 4.15E-5 -6.62E-5
ADPE [kg Sb-Eq.] 7.00E-5 3.13E-6 2.09E-7 0.00E+0 1.82E-8 2.64E-6 6.99E-7 -1.31E-6
ADPF [MJ] 7.77E+1 1.72E+0 2.93E-1 0.00E+0 4.76E-3 1.46E+0 5.10E-1 -9.11E+0
GWP = Global warming potential; ODP = Depletion potential of the stratospheric ozone layer; AP = Acidification potential of land and water; EP =
Caption Eutrophication potential; POCP = Formation potential of tropospheric ozone photochemical oxidants; ADPE = Abiotic depletion potential for non-
fossil resources; ADPF = Abiotic depletion potential for fossil resources
RESULTS OF THE LCA - INDICATORS TO DESCRIBE RESOURCE USE according to EN 15804+A1: 1 m2
Natural Wood, 25 mm, painted finish, delivered and used in Denmark
Parameter Unit A1-A3 A4 A5 B1 C1 C2 C4 D
PERE [MJ] 6.54E+1 2.47E-2 1.60E-1 0.00E+0 3.91E-2 2.08E-2 8.45E+0 -1.76E+0
PERM [MJ] 7.36E+1 0.00E+0 0.00E+0 0.00E+0 0.00E+0 0.00E+0 0.00E+0 0.00E+0
PERT [MJ] 1.39E+2 2.47E-2 1.60E-1 0.00E+0 3.91E-2 2.08E-2 8.45E+0 -1.76E+0
PENRE [MJ] 8.09E+1 1.76E+0 4.58E-1 0.00E+0 4.31E-2 1.49E+0 6.68E-1 -9.58E+0
PENRM [MJ] 1.53E-1 0.00E+0 0.00E+0 0.00E+0 0.00E+0 0.00E+0 0.00E+0 0.00E+0
PENRT [MJ] 8.10E+1 1.76E+0 4.58E-1 0.00E+0 4.31E-2 1.49E+0 6.68E-1 -9.58E+0
SM [kg] 2.23E-2 0.00E+0 3.10E-2 0.00E+0 0.00E+0 0.00E+0 0.00E+0 0.00E+0
RSF [MJ] 2.03E-4 0.00E+0 0.00E+0 0.00E+0 0.00E+0 0.00E+0 0.00E+0 0.00E+0
NRSF [MJ] 3.20E-5 0.00E+0 0.00E+0 0.00E+0 0.00E+0 0.00E+0 0.00E+0 0.00E+0
FW [m³] 5.44E-1 2.99E-4 1.30E-4 0.00E+0 1.19E-5 2.52E-4 2.81E-4 -6.39E-4
PERE = Use of renewable primary energy excluding renewable primary energy resources used as raw materials; PERM = Use of
renewable primary energy resources used as raw materials; PERT = Total use of renewable primary energy resources; PENRE = Use of
non-renewable primary energy excluding non-renewable primary energy resources used as raw materials; PENRM = Use of non-
Caption
renewable primary energy resources used as raw materials; PENRT = Total use of non-renewable primary energy resources; SM = Use
of secondary material; RSF = Use of renewable secondary fuels; NRSF = Use of non-renewable secondary fuels; FW = Use of net fresh
water
RESULTS OF THE LCA – WASTE CATEGORIES AND OUTPUT FLOWS according to EN 15804+A1:
1 m2 Natural Wood, 25 mm, painted finish, delivered and used in Denmark
Parameter Unit A1-A3 A4 A5 B1 C1 C2 C4 D
HWD [kg] 5.66E-2 1.77E-3 1.51E-3 0.00E+0 5.40E-5 1.50E-3 1.48E-3 -5.82E-2
NHWD [kg] 1.72E+0 1.22E-1 1.15E-1 0.00E+0 1.12E-3 1.03E-1 6.20E-2 -1.98E+0
RWD [kg] 1.01E-4 1.20E-5 2.54E-6 0.00E+0 5.78E-7 1.01E-5 4.98E-6 -2.41E-5
CRU [kg] 6.83E-6 0.00E+0 0.00E+0 0.00E+0 0.00E+0 0.00E+0 0.00E+0 0.00E+0
MFR [kg] 1.56E-2 0.00E+0 0.00E+0 0.00E+0 0.00E+0 0.00E+0 0.00E+0 0.00E+0
MER [kg] 8.70E-3 0.00E+0 0.00E+0 0.00E+0 0.00E+0 0.00E+0 0.00E+0 0.00E+0
EEE [MJ] 0.00E+0 0.00E+0 0.00E+0 0.00E+0 0.00E+0 0.00E+0 1.73E+0 0.00E+0
EET [MJ] 0.00E+0 0.00E+0 0.00E+0 0.00E+0 0.00E+0 0.00E+0 5.57E+0 0.00E+0
HWD = Hazardous waste disposed; NHWD = Non-hazardous waste disposed; RWD = Radioactive waste disposed; CRU = Components
Caption for re-use; MFR = Materials for recycling; MER = Materials for energy recovery; EEE = Exported electrical energy; EEE = Exported
thermal energy
6. LCA: Interpretation
The estimated impact results are only relative and use of cement, wood, and paint in the foreground
statements which do not indicate the end points of the processes. Global Warming Potential net emissions
impact categories, exceeding threshold values, safety share is much larger in C4 than in A1-A3 (see why in
margins or risks. chart (2)), while other impact categories in module D in
general are avoided in the waste system owing to the
Two charts are presented: (1) with the standard incineration of end-of-life panels and substitution of
lifecycle impact categories displaying the share of natural gas and Danish electricity mix. C4 also slightly
impacts across all lifecycle stages, and (2) displaying follows emissions of compounds associated to other
the total carbon balance of the Troldekt product's impact categories. A relatively inefficient transportation
lifecycle system. of end-of-life panels to waste incineration causes
emissions in especially Abiotic depletion of non-fossil
Impacts from the A1-A3 modules are dominant in the resources, Depletion of stratospheric ozone, and
life cycle of the Troldtekt Natural Wood painted panel Photochemical ozone formation.
products. This is primarily caused by the acquisition
The embodied emissions associated to the raw sequestered in A1-A3 and some fossil CO taken up in
2
materials (primarily cement and paint) are the main A1-A3 and B1 is re-emitted in C4. CO emissions
2-eq
cause of impacts, especially in terms of net Global occuring in the remaining modules are negligible.
Warming Potential, with respectively 7,7 kg CO and
2-eq
0,4 kg CO followed by minor impacts from additives. The amount of wood stored in the product refers to a
2-eq
In general, direct emissions from the Troldtekt negative contribution to Global Warming Potential,
production site are relatively small. Abiotic depletion of reducing the share of Global Warming Potential in A1-
fossil resources appears from the burden of producing A3. This is due to the sequestration of biogenic carbon
cement using fossil raw material such as limestone of wood during tree growth. The sequestered carbon
and to a large extent fossil fuels. In terms of carbon does not contribute to global warming as long as it is
balance, biogenic CO in A1-A3 offsets nearly all the stored in the biomass.
2
fossil CO emissions in A1-A3. All biogenic CO
2 2
8 Environmental Product Declaration Troldtekt A/S – Troldtekt 25mm Natural Wood - painted
for Photochemical ozone formation, Acidification,
Global Warming and Eutrophication, by order of
Summary importance. The treatment of wastewater from the
Within the cradle to grave, the following aspects have painting cabin also contributes significantly to potential
been identified as major contributors, mainly in the impacts in terms of Eutrophication.
categories Global Warming Potential and Abiotic
depletion of fossil resources: The clinker (cement) production is the most critical
process of the Troldtekt product system, but
 Emissions from the clinker production from inaccuracies around the amount used will not
material invalidate the present conclusions.
 Emissions from the clinker production from
Notably, by introducing cements with less carbon
fuel
footprint into production, as well as improved paint
 Substituted emissions from end of life consumption management, could lead to significant
incineration reductions of especially the Global Warming Potential
indicator.
Additionally, for painted panels, the manufacture of
paint contribute significantly to impacts on potentials
7. Requisite evidence
7.3 VOC emissions
7.1 Testing of substances used Testing for VOC emissions has been conducted in
A detailed assessment of substances used was accordance with EN ISO 16000-6. Analysis of the air
conducted by a DAkkS-accredited laboratory, based sampled on Tenax was performed at the Danish
on a sample (prepared according to EN 15443), Technological Institute under DANAK accreditation
available in the Test Report 2018P216294, using 392. Report no. MAIC-2019-1418. Reporting of
inductively coupled plasma mass spectrometry (EN measured concentrations in toluene equivalents
16171) and X-ray fluorescence (EN 15309), for the according to EN 16516. This test is basis for the Finish
following: M1 Material certificate as well as the Danish Indoor
 Heavy metals (cadmium, mercury, etc.) Climate labeling certificate.
 and other elements
AgBB overview of results (28 days [µg/m³])
Name Value Unit
7.2 Leaching TVOC (C6 - C16) 12 μg/m3
No leaching measurement was conducted according Sum SVOC (C16 - C22) 0 - 5 μg/m3
to EN 717-1. VOC without NIK 0 - 5 μg/m3
Carcinogenic Substances 1 μg/m3
8. References
Standards DIN EN ISO 14025
DIN EN ISO 14025:2011, Environmental labels and
AgBB declarations – Type III environmental
AgBB, Ausschuss zur gesundheitlichen Bewertung von declarations – Principles and procedures, German and
Bauprodukten (Committee for Health-related English versions EN ISO 14025:2011
Evaluation of Building Products)
EN 13168
BBSR EN 13168:2012+A1:2015, Thermal insulation products
BBSR, Bundesinstitut für Bau-, Stadt- und for buildings. Factory made wood wool (WW) products.
Raumforschung (Federal Institute for Research on Specification
Building, Urban Affairs and Spatial Development).
BBSR table: EN 13964
https://www.nachhaltigesbauen.de/fileadmin/pdf/baust EN 13964:2014, Suspended ceilings. Requirements
off_gebauededaten/BNB_Nutzungsdauern_von_Bautei and test methods
len_2017-02-24.pdf
EN 15309
DIN 4108-4 EN 15309:2007, Characterization of waste and soil.
DIN 4108-4:2017-03, Thermal insulation and energy Determination of elemental composition by X-ray
economy in buildings - Part 4: Hygrothermal design fluorescence
values
EN 15443
DIN 52612-2 EN 15443:2011, Solid recovered fuels. Methods for the
DIN 52612-2, Testing of thermal insulating materials; preparation of the laboratory sample
determination of thermal conductivity by means of the
guarded hot plate apparatus; conversion of the EN 15804
measured values for building applications. 1 June 1984 EN 15804:2012, EN 15804:2012+A1 2013,
Sustainability of construction works – Environmental
9 Environmental Product Declaration Troldtekt A/S – Troldtekt 25mm Natural Wood - painted
Product Declarations – Core rules for the product
category of construction products. Product Category Rule A
Product Category Rule A, IBU, 2019, Part A,
EN 16171 Calculation Rules for the Life Cycle Assessment and
EN 16171:2016, Sludge, treated biowaste and soil. Requirements on the Project Report. v.1.8. IBU, 2019.
Determination of elements using inductively coupled
plasma mass spectrometry (ICP-MS) Product Category Rule B
Product Category Rule B, IBU, 2019, Part B,
EN 16449 Requirements on the EPD for Wood cement - Mineral-
EN 16449:2014, EN 16449:2014, Wood and wood- bonded wooden composites. v.1.7. IBU, 2019.
based products - Calculation of the biogenic carbon
content of wood and conversion to carbon dioxide
Further References
EN 16516
EN 16516:2017+A1:2020, Construction products: General Programme Instructions, IBU 2016
Assessment of release of dangerous substances. General Programme Instructions for the Preparation of
Determination of emissions into indoor air EPDs at the Institut Bauen und Umwelt e.V. Version 1.,
Berlin: Institut Bauen und Umwelt e.V., 2016.
EN 717-1
EN 717-1:2004, Wood-based Panels – Determination Software/database
of Formaldehyde Release – Formaldehyde emission OneClick LCA software, Pre-verified EPD tool,
by the chamber method Bionova: https://www.oneclicklca.com/
ISO 16000-6 Database: Ecoinvent v.3.6. cut-off (2019)
ISO 16000-6:2011, Indoor air - Part 6: Determination of
volatile organic compounds in indoor and test chamber
air by active sampling on Tenax TA sorbent, thermal
desorption and gas chromatography using MS or MS-
FID
10 Environmental Product Declaration Troldtekt A/S – Troldtekt 25mm Natural Wood - painted
Publisher
Institut Bauen und Umwelt e.V. Tel +49 (0)30 3087748- 0
Panoramastr. 1 Fax +49 (0)30 3087748- 29
10178 Berlin Mail info@ibu-epd.com
Germany Web www.ibu-epd.com
Programme holder
Institut Bauen und Umwelt e.V. Tel +49 (0)30 - 3087748- 0
Panoramastr 1 Fax +49 (0)30 – 3087748 - 29
10178 Berlin Mail info@ibu-epd.com
Germany Web www.ibu-epd.com
Author of the Life Cycle
Assessment Tel 98777223
Aalborg Portland Fax 80815733
Rørdalsvej 44 Mail
92200 Aalborg Ø stefan.e.danielsson@cementirhol
Denmark ding.it
Web www.aalborgportland.dk
Owner of the Declaration
Troldtekt A/S Tel +45 8747 8100
Sletvej 2A Fax +45 8747 8111
8310 Tranbjerg J Mail sales@troldtekt.dk
Denmark Web https://www.troldtekt.com
