ENVIRONMENTAL PRODUCT DECLARATION
as per ISO 14025 and EN 15804+A1
Owner of the Declaration Stiferite
Publisher Institut Bauen und Umwelt e.V. (IBU)
Programme holder Institut Bauen und Umwelt e.V. (IBU)
Declaration number EPD-STF-20200237-CBA3-EN
Issue date 18.12.2020
Valid to 17.12.2025
stiferite GTM average thick panel
Stiferite
www.ibu-epd.com | https://epd-online.com
General Information
Stiferite stiferite GTM average thick panel
Programme holder Owner of the declaration
IBU – Institut Bauen und Umwelt e.V. Stiferite
Hegelplatz 1 Viale Navigazione Interna 54
10117 Berlin 35129 Padova
Germany Italy
Declaration number Declared product / declared unit
EPD-STF-20200237-CBA3-EN STIFERITE GTM expanded rigid polyurethane foam, covered on both
sides by multilayer facer based on aluminium, facers, and produced by
Stiferite. The EPD applies to 1 m2 of average 61 mm thickness PUR
sandwich board, i.e. 0.061 m3, with an average density between foam and
facing of 34.7 kg/m3.
This declaration is based on the product category rules: Scope:
Insulating materials made of foam plastics, 01.08.2021 Stiferite produces STIFERITE GTM that is a high performance insulation
(PCR checked and approved by the SVR) board manufactured from closed cell expanded rigid polyurethane foam,
covered on both sides by multilayer facers based on aluminium.The data
have been provided by the only Stiferite factory that is located in Padova
Issue date (Italy) for the year 2019.
The owner of the declaration shall be liable for the underlying information
18.12.2020
and evidence; the IBU shall not be liable with respect to manufacturer
information, life cycle assessment data and evidences.
Valid to
The EPD was created according to the specifications of EN 15804+A1. In
17.12.2025 the following, the standard will be simplified as EN 15804.
Verification
The standard EN 15804 serves as the core PCR
Independent verification of the declaration and data according to ISO
14025:2011
internally X externally
Dipl.-Ing. Hans Peters
(Chairman of Institut Bauen und Umwelt e.V.)
Dipl.-Ing. Hans Peters Prof. Dr. Birgit Grahl,
(Managing Director Institut Bauen und Umwelt e.V.) (Independent verifier)
1 Environmental Product Declaration - Stiferite - stiferite GTM average thick panel
Product
Name Value Unit
Product description/Product definition
Gross density 34.7 kg/m3
STIFERITE'S thermo insulation panels are mainly used in the
building/construction sector and that of industrial insulation. Declared Thermal conductivity λD acc. to /EN 0.023 W/mK
The panels are made of thermo-setting closed cells 13165/
polyurethane foam (PU) supplied with various types of flexible Compressive strength at 10% deformation acc. to
> 150 kPa
facers on both sides of the panel. The nature/type of facer /EN 826/
contributes to the performance characteristics of the product Tensile strength perpendicular to the face acc. to
> 35 kPa
and its application. /EN 1607/
Expanded rigid polyurethane foam is distinguished by its'
Water absorption by total immersion acc. to /EN Vol.-
excellent thermo insulation performance, mechanical < 1
12087/ %
resistance, workability, lightness, and durability.
Water absorption by partial immersion acc. to /EN
< 0.1 kg/m²
1609/
The performance of STIFERITE'S panels is determined based
Water vapour diffusion resistance factor μ acc. to
on the European norm EN 13165:2012+A2:2016 Thermal 146
/EN 12086/
insulation products for buildings - Factory made rigid
polyurethane foam (PU) products - Specification. Euroclass reaction to fire acc. to /EN 11925/ F
This EPD refers to STIFERITE's GTM average thick panel,
This provides a thermal resistance R = 2.65 m² k/W.
made of an insulation component in polyurethane foam using
blowing agent Pentane-based, covered on both sides with
multilayer facers based on aluminium.
Base materials/Ancillary materials
The gas-tight properties of the facing allow the highest thermal Core material (about 83.7 % of the weight of the declared
insulation to be achieved and maintained over time. The panel unit):
is produced in standard dimensions of 600 x 1200 mm and Closed-cell Polyiso (PIR) rigid foam made from MDI (50-65 %),
straight finished edges. Upon request and for minimum polyols (20-30 %), pentane (4-5 %) and additives (4-7 %).
quantities, the panels may be produced in various dimensions, Facing (about 16.3 % of the weight of the declared unit):
and the borders may be rabbeted along the sides. The surface multilayer facer consisting of PE and PP (20-40 %), aluminium
of the panel may be evened off by sandpaper in order to allow (10-15%) and paper (55-75%).
installation to uneven surfaces. STIFERITE GTM panel is
produced by a certified company with systems: ISO 9001, /SO The PU board for insulation:
45001, ISO 14001 in its entire line of products. For the placing
• This product/article/at least one partial article contains
on the market of the product in the European Union/European
substances listed in the candidate list (date: 17.11.2020)
Free Trade Association (EU/EFTA) (with the exception of
exceeding 0.1 percentage by mass: no
Switzerland) Regulation (EU) No. 305/2011 (CPR) applies. The
• This product/article/at least one partial article doesn't
product needs a Declaration of Performance (DoP) taking into
contain other CMR substances in categories 1A or 1B
consideration EN 13165:2012+A2:2016 Thermal insulation
which are not on the candidate list, exceeding 0.1
products for building- factory made rigid polyurethane foam
percentage by mass: no
(PU) products - Specification and the CE-marking. For the
• Biocide products were added to this construction
application and use the respective national provisions apply.
product or it has been treated with biocide products (this
Application then concerns a treated product as defined by the (EU)
Ordinance on Biocide Products No. 528/2012): no
The STIFERITE GTM panel is
Additional declaration according to quoted law: The product is
recommended for insulaing: wall, floor and roof insulation under
compliant with all requirements indicated at Additional
waterproof membrane with cold applied.
declaration according to quoted law: The product is compliant
STIFERITE GTM is used to make Stiferite GT3, GT4, GT5 and
with all requirements indicated in chapter 2.5.7 'Isolanti termici
GT6 products.
ed acustici' of the n.256 D.L. of the 23th June 2022 (CAM
Technical Data EDILIZIA):
The data provided by the Declaration of Performance apply. In • Any blowing agent with Ozone depletion potential >0 is
this Life Cycle Assessment, a PU insulation board with the not used in production
following properties has been regarded: • Any substances of Very High Concern-SVHC in
Constructional data concentration of more than 0,1 %w are not used in
production (REACH n. 1907/2006). Any specific
authorizations for use are eserved provided for by the
same Regulation for the substances included in Annex
XIV and specifications restrictions set out in Annex XVII
of the Regulation.
• Catalysts lead-based are not used in production
• Flame retardants used in production (belonging to the
Organophosphorus class) are not banned by any
national or European regulation
• According to the raw materials declarations of suppliers
the minimum amount of recycled raw materials based
on the insulation board (PU foam and facers) weight is 3
%w and the minimum amount of recycled raw materials
based on the PU insulation foam weight is 4 %w (note:
2 Environmental Product Declaration - Stiferite - stiferite GTM average thick panel
this information is not explicitly considered in the LCA The durability of insulation panels is normally at least as long as
and not included in the EPD tables that only refer to the lifetime of the building in which it is used. The experimental
recycling content in the foreground system). data show that the reference life is longer than 50 years, Clima
2019.
Reference service life
LCA: Calculation rules
gate with options). It also includes the transport to the
Declared Unit construction site, the installation and the end-of-life stage of the
The declared unit is 1 m² with an average thickness of 61 mm, used PU thermal insulation board. The life cycle is split into the
e. g. 0.061 m³. following individual phases:
Corresponding conversion factors are listed in the table below. A1 - Raw material formulation
Declared unit A2 - Raw material transport
A3 - Production of the insulation board and packaging material
Name Value Unit
A4 - Transport to the construction site
Declared unit 1 m2 A5 - Emissions and cutting losses during installation and
Gross density 34.7 kg/m3 packaging disposal
Volume 0.061 m³ C2 - Transport to end of life
C3/C4 - End-of-Life: waste management (thermal recovery,
Grammage 212 kg/m2
landfill)
Declared thermal conductivity λD 0.023 W/mK D - Benefits and loads beyond system boundary
Layer thickness 0.061 m
Geographic Representativeness
Conversion factor to 1 kg 2.12 kg/m²
Land or region, in which the declared product system is
Weight of declared unit 2.12 kg/m²
manufactured, used or handled at the end of the product´s
The LCI data used in this report refer to an average product lifespan: Italy
having an average thickness (materials in the recipes of
different thicknesses are weighted according to the relative
production in square meters). The type of declaration is 1 c - Comparability
declaration of an average product from a manufacturer's plant. Basically, a comparison or an evaluation of EPD data is only
possible if all the data sets to be compared were created
according to EN 15804 and the building context, respectively
the product-specific characteristics of performance, are taken
System boundary into account. For life cycle modelling of the considered
This life cycle assessment for the production of the products, the GaBi 9 2020 has been used.
polyurethane insulation board considers the life cycle from the
supply of raw materials to the manufacturer´s gate (cradle-to-
LCA: Scenarios and additional technical information
The results for the end-of-life are declared for the 2 different
scenarios:
Name Value Unit
Transport to the building site (A4) Scenario No 1: Material Incineration 100 %
The distances calculated are weighted average distances Scenario No 2: Landfill 100 %
according to the overall sales distribution; such distribution is
C4: Disposal scenarios used is divided into the 2
considered similar for all Stiferite products.
sub-scenarios:
Name ValueUnit
1) Incineration 100% (C4/1)
Truck with a capacity of 17.3 tons 271 km 2) Landfilling 100% (C4/2)
Ferry with a capacity of 1200-10000 dwt payload
144 km
capacity D: Benefits and loads beyond system boundary is divided into
Ship with a capacity of 27500 dwt payload capacity the 2 sub-scenarios:
tons 11000 km 1) Incineration 100% (D1)
2) Landfilling 100% (D2)
Plane with a capacity of 22 ton 0 km
Installation into the building (A5) Reuse, recovery and/or recycling potentials (D), relevant
Name Value Unit scenario information
Material loss 0.0423 kg Name Value Unit
VOC in the air Pentane 1.27E-06 kg Module D includes credits from recycling materials of insulation
panels and packaging, energy credits from thermal recovery of
the packaging. The results are declared for the same 3 different
End of life (C1-C4)
scenarios described above.
3 Environmental Product Declaration - Stiferite - stiferite GTM average thick panel
LCA: Results
The tables below show the results of the LCA. Basic information on all declared modules provides chapter 4.
There are two scenarios for the end-of-life (C3, C4 and D) analyzed: Scenario 1 considers 100% incineration, Scenario 2 considers
100% landfill disposal.
For SM, RSF, NRSF,CRU indicators only the foreground system is considered.
DESCRIPTION OF THE SYSTEM BOUNDARY (X = INCLUDED IN LCA; MND = MODULE NOT DECLARED; MNR = MODULE NOT
RELEVANT)
Benefits and
Construction loads beyond
Product stage Use stage End-of-life stage
process stage the system
boundaries
la ire ta m w a Ry lp p u s tro p s n a rT g n iru tc a fu n a M e h t m o rf tro p s n a rTe tis e h t o t e ta g y lb m e s s A e s U e c n a n e tn ia M ria p e R tn e m e c a lp e R tn e m h s ib ru fe R y g re n e la n o ita re p Oe s u re ta w la n o ita re p Oe s u n o itc u rts n o c -e Dn o itilo m e d tro p s n a rT g n is s e c o rp e ts a W la s o p s iD -e s u e R-y re v o c e R-g n ilc y c e Rla itn e to p
A1 A2 A3 A4 A5 B1 B2 B3 B4 B5 B6 B7 C1 C2 C3 C4 D
X X X X X MND MND MNR MNR MNR MND MND MND X X X X
RESULTS OF THE LCA - ENVIRONMENTAL IMPACT according to EN 15804+A1: 1 m² GTM average thick panel
Parameter Unit A1-A3 A4 A5 C2 C3/1 C3/2 C4/1 C4/2 D/1 D/2
GWP kg CO 2 eq 5.47E+00 1.73E-01 9.77E-03 9.77E-03 0 0 4.31E+00 2.23E-01 -2.39E+00 -6.35E-02
ODP kg CFC11 eq 9.54E-06 1.91E-07 7.06E-14 7.06E-14 0 0 5.33E-11 3.96E-11 -1.31E-09 -1.42E-11
AP kg SO 2 eq 1.44E-02 3.38E-04 2.44E-05 2.44E-05 0 0 1.79E-03 3.78E-04 -5.46E-03 -1.08E-04
EP kg PO 43 eq 1.95E-03 4.81E-05 5.66E-06 5.66E-06 0 0 4.24E-04 9.45E-05 -5.08E-04 -1.16E-05
POCP kg Ethen eq 3.59E-03 7.59E-05 -6.73E-06 -6.73E-06 0 0 1.22E-04 6.22E-05 -4.38E-04 -1.35E-05
ADPE kg Sb eq 1.32E-05 2.73E-07 7.3E-10 7.3E-10 0 0 5.76E-08 3.16E-08 -6.25E-07 -1.74E-08
ADPF MJ 1.32E+02 2.79E+00 1.34E-01 1.34E-01 0 0 1.66E+00 1.16E+00 -2.94E+01 -1.39E+00
GWP = Global warming potential; ODP = Depletion potential of the stratospheric ozone layer; AP = Acidification potential of land and water; EP =
Eutrophication potential; POCP = Formation potential of tropospheric ozone photochemical oxidants; ADPE = Abiotic depletion potential for non-fossil
resources; ADPF = Abiotic depletion potential for fossil resources
RESULTS OF THE LCA - INDICATORS TO DESCRIBE RESOURCE USE according to EN 15804+A1: 1 m² GTM average thick
panel
Parameter Unit A1-A3 A4 A5 C2 C3/1 C3/2 C4/1 C4/2 D/1 D/2
PERE MJ 2.01E+01 IND 4.34E-01 IND IND IND 3.93E-01 IND IND IND
PERM MJ 1.82E-02 IND -1.1E-02 IND IND IND 0 IND IND IND
PERT MJ 2.01E+01 2.71E-02 4.23E-01 7.75E-03 0 0 3.93E-01 3.25E-01 -9.07E+00 -1.69E-01
PENRE MJ 6.77E+01 IND 2.16E+00 IND IND IND 7.21E+01 IND IND IND
PENRM MJ 7.19E+01 IND -1.97E+00 IND IND IND -6.99E+01 IND IND IND
PENRT MJ 1.4E+02 6E-01 1.86E-01 1.35E-01 0 0 2.17E+00 1.54E+00 -4.16E+01 -1.55E+00
SM kg 0 0 0 0 0 0 0 0 0 0
RSF MJ 0 0 0 0 0 0 0 0 0 0
NRSF MJ 0 0 0 0 0 0 0 0 0 0
FW m3 4.22E-02 6.69E-05 1.01E-03 1.92E-05 0 0 1.05E-02 5.11E-04 -1.4E-02 -2.67E-04
PERE = Use of renewable primary energy excluding renewable primary energy resources used as raw materials; PERM = Use of renewable primary
energy resources used as raw materials; PERT = Total use of renewable primary energy resources; PENRE = Use of non-renewable primary energy
excluding non-renewable primary energy resources used as raw materials; PENRM = Use of non-renewable primary energy resources used as raw
materials; PENRT = Total use of non-renewable primary energy resources; SM = Use of secondary material; RSF = Use of renewable secondary fuels;
NRSF = Use of non-renewable secondary fuels; FW = Use of net fresh water
RESULTS OF THE LCA – WASTE CATEGORIES AND OUTPUT FLOWS according to EN 15804+A1:
1 m² GTM average thick panel
Parameter Unit A1-A3 A4 A5 C2 C3/1 C3/2 C4/1 C4/2 D/1 D/2
HWD kg 9.97E-06 3.5E-08 2.01E-07 1.01E-08 0 0 2.04E-09 1.07E-08 -2.28E-08 -1.36E-09
NHWD kg 2.14E-01 4.09E-05 6.03E-02 1.16E-05 0 0 3.55E-02 1.97E+00 -2.05E-02 -3.95E-04
RWD kg 3.25E-03 1.16E-06 7.58E-05 2.89E-07 0 0 2.03E-04 1.52E-04 -4.86E-03 -6.34E-05
CRU kg 2.55E-03 0 5.1E-05 0 0 0 0 0 0 0
MFR kg 0 0 1.76E-02 0 0 0 0 0 0 0
MER kg 0 0 1.96E-02 0 0 0 2E+00 0 0 0
EEE MJ 0 0 9.57E-02 0 0 0 1.41E+01 4.82E-02 0 0
EET MJ 0 0 2.18E-01 0 0 0 7.13E+00 0 0 0
HWD = Hazardous waste disposed; NHWD = Non-hazardous waste disposed; RWD = Radioactive waste disposed; CRU = Components for re-use;
MFR = Materials for recycling; MER = Materials for energy recovery; EEE = Exported electrical energy; EET = Exported thermal energy
Disclaimer 1 – for the indicator 'Potential Human exposure efficiency relative to U235'. This impact category deals mainly with the
4 Environmental Product Declaration - Stiferite - stiferite GTM average thick panel
eventual impact of low-dose ionizing radiation on human health of the nuclear fuel cycle. It does not consider effects due to possible
nuclear accidents, occupational exposure or radioactive waste disposal in underground facilities. Potential ionizing radiation from the
soil, radon and from some construction materials is also not measured by this indicator.
Disclaimer 2 – for the indicators 'abiotic depletion potential for non-fossil resources', 'abiotic depletion potential for fossil resources',
'water (user) deprivation potential, deprivation-weighted water consumption', 'potential comparative toxic unit for ecosystems', 'potential
comparative toxic unit for humans – cancerogenic', 'Potential comparative toxic unit for humans - not cancerogenic', 'potential soil
quality index'. The results of this environmental impact indicator shall be used with care as the uncertainties on these results are high
as there is limited experience with the indicator.
References
Standards EN 12086: 2013 Thermal insulating products for building
applications. Determination of water vapour transmission
EN 15804 properties.
EN 15804:2012-04+A1 2013, Sustainability of construction
works — Environmental Product Declarations — Core rules for EN 11925
the product category of construction products. EN 11925:2010 Reaction to fire tests. Ignitability of products
subjected to direct impingement of flame. Single-flame source
ISO 14025 test.
EN ISO 14025:2011-10, Environmental labels and declarations
— Type III environmental declarations — Principles and Further References
procedures.
BNB
IBU 2016 Bewertungssystem Nachhaltiges Bauen (en: assessment
Institut Bauen und Umwelt e.V.: General Programme system sustainable building)
Instructions for the Preparation of EPDs at the Institut Bauen https://www.bbsr.bund.de/BBSR/EN/RP/FutureBuilding/2SustainableBuildingQuality/2009/ServiceLife/01_Start_dossier.html?
und Umwelt e.V. Version 1., Berlin: Institut Bauen und Umwelt n=391866&notFirst=true&docId=390900
e.V., 2016.
www.ibu-epd.com Candidate List
https://echa.europa.eu/it/candidate-list-table (date 17.11.2020)
ISO 9001
ISO 9001:2015 Quality management Clima 2019
Clima 2019 PaperPolyurethane 'Environmental Impacts for a
ISO 14001 Polyurethane Panel' E. Guolo, F. Cappelletti, P. Romagnoni, F.
ISO 14001: 2015 Environmental management systems Raggiotto
ISO 45001 GaBi 9 2020
ISO 45001: 2018 Occupational health and safety management GaBi 8: Documentation of GaBi 8: Software-System and
systems Database for Life Cycle Engineering. Copyright, TM. Stuttgart,
Leinfelden-Echterdingen, 1992-2020
EN 13165 http://www.gabi-software.com
EN 13165:2012+A2:2016 Thermal insulation products for
buildings - Factory made rigid polyurethane foam (PU) PANGPP 2017
products - Specification Piano d' Azione Nazionale sul Green Public Procurement
(PANGPP) – Gazzetta Ufficiale della Repubblica Italiana, Serie
EN 826 Generale n.17, 11-10-2017,
EN 826:2013 Determination of Compression Behavior of http://www.minambiente.it/sites/default/files/archivio/allegati/GPP/GPP_CAM_Edilizia.pdf
Thermal Insulation Products
PCR Part A
EN 1607 Product Category Rules for Building-Related Products and
EN 1607: 2013 Thermal insulating products for building Services. Part A: Calculation Rules for the Life Cycle
applications. Determination of tensile strength perpendicular to Assessment and Requirements on the Background Report.
faces Version 06.2017.
EN 12087 PCR Part B
EN 12087:2013 Thermal insulating products for building PCR Guidance-Texts for Building-Related Products and
applications. Determination of long term water absorption by Services; Part B: Requirements on the EPD for Insulating
immersion. materials made of foam plastics; Institute Construction and
Environment e.V. (IBU). Version 06.2017
EN 1609 https://epd-online.com
EN 1609: Thermal insulating products for building applications.
Determination of short term water absorption by partial REACH
immersion. REACH Registration, Evaluation, Authorization and Restriction
of Chemical, 2007
EN 12086
5 Environmental Product Declaration - Stiferite - stiferite GTM average thick panel
Publisher
Institut Bauen und Umwelt e.V. +49 (0)30 3087748- 0
Hegelplatz 1 info@ibu-epd.com
10117 Berlin www.ibu-epd.com
Germany
Programme holder
Institut Bauen und Umwelt e.V. +49 (0)30 3087748- 0
Hegelplatz 1 info@ibu-epd.com
10117 Berlin www.ibu-epd.com
Germany
Author of the Life Cycle Assessment
thinkstep Italy +39 0544 467132
Via Bovini 43 info@thinkstep.com
48123 Ravenna www.thinkstep.com
Italy
Owner of the Declaration
Stiferite +39 049 8997911
Viale Navigazione Interna 54 info@stiferite.com
35129 Padova www.stiferite.com
Italy
6 Environmental Product Declaration - Stiferite - stiferite GTM average thick panel
