ENVIRONMENTAL PRODUCT DECLARATION
as per ISO 14025 and EN 15804+A2
Owner of the Declaration SOUDAL N.V.
Publisher Institut Bauen und Umwelt e.V. (IBU)
Programme holder Institut Bauen und Umwelt e.V. (IBU)
Declaration number EPD-SDL-20240122-CAA1-EN
Issue date 03.04.2024
Valid to 16.01.2028
SOUDAFIX VE400-SF
SOUDAL N.V.
www.ibu-epd.com | https://epd-online.com
General Information
SOUDAL N.V. SOUDAFIX VE400-SF
Programme holder Owner of the declaration
IBU – Institut Bauen und Umwelt e.V. SOUDAL N.V.
Hegelplatz 1 Everdongenlaan 18-20
10117 Berlin 2300 Turnhout
Germany Belgium
Declaration number Declared product / declared unit
EPD-SDL-20240122-CAA1-EN The declared product is the two-component reaction resin mortar
"SOUDAFIX VE400-SF", manufacturated by SOUDAL N.V.. The declared
unit is based on 1 kg reaction resin product in the ratio at which the two
components must be mixed before use. The packaging is also included in
the calculation, since the product is sold by SOUDAL N.V. with its
packaging. The declared unit is indicated in [kg].
This declaration is based on the product category rules: Scope:
Reaction resin products, 01.08.2021 This document covers the two-component reaction resin mortar
(PCR checked and approved by the SVR) "SOUDAFIX VE400-SF". To prepare the life cycle assessment [LCA],
specific data were collected from the SOUDAL N.V. manufacturing facility
in Germany. The assessment is based on data from 2020 which
Issue date correspond to the yearly average. The procedure by which the data are
allocated to the declared unit is described in the "Allocation" section.
03.04.2024
Valid to
16.01.2028 The owner of the declaration shall be liable for the underlying information
and evidence; the IBU shall not be liable with respect to manufacturer
information, life cycle assessment data and evidences.
The EPD was created according to the specifications of EN 15804+A2. In
the following, the standard will be simplified as EN 15804.
Verification
The standard EN 15804 serves as the core PCR
Independent verification of the declaration and data according to ISO
14025:2011
Dipl.-Ing. Hans Peters internally X externally
(Chairman of Institut Bauen und Umwelt e.V.)
Florian Pronold Angela Schindler,
(Managing Director Institut Bauen und Umwelt e.V.) (Independent verifier)
1 Environmental Product Declaration - SOUDAL N.V. - SOUDAFIX VE400-SF
Product
Gel and working time:
Product description/Product definition -10°C 90 min.
The declared product SOUDAFIX VE400-SF is a two- -5°C 90 min.
component reaction resin mortar based on vinyl ester resin that 0°C 45 min.
is delivered in a two-component plastic cartridge. The high- +5°C 25 min.
performance product is applied through a static mixer using a +10°C 15 min.
manual, battery-operated or pneumatic gun. It was specially +20°C 6 min.
developed for use in securing threaded rods, rebar or internally +30°C 4 min.
threaded sleeves in solid brick, concrete, autoclaved aerated +35°C 2 min.
concrete and lightweight concrete. Due to its excellent +40°C 1.5 min.
mechanical strength, it can also be used in perforated brick by
using a special perforated sleeve. SOUDAFIX VE400-SF Curing time in dry substrate:
mortar has a wide range of possible applications at installation -10°C 1440 min.
tempeartures as low as -10 °C and operating temperatures of -5°C 840 min.
up to 120 °C, and offers high chemical resistance in extreme 0°C 420 min.
environments like swimming pools (chlorine) or near the sea +5°C 120 min.
(salt). With its broad range of national and international +10°C 80 min.
approvals and certifications, it can be used in almost any +20°C 45 min.
application. +30°C 25 min.
+35°C 20 min.
Marketing of the product in the EU/EFTA (except for +40°C 15 min.
Switzerland) is governed by Regulation (EU) No. 305/2011
(CPR). The product requires a Declaration of Performance
subject to ETA-10/0167, ETA-21/0170, ETA-12/0558 and CE
marking. For more information, please refer to the relevant technical data
sheet.
Product performance values in accordance with the Declaration
Application
of Performance with regard to its principal charateristics
The declared product SOUDAFIX VE400-SF is used to reliably according to ETA-10/0167, ETA-21/0170 and ETA-12/0558.
secure threaded rods, internally threaded sleeves and post-
installed rebar connections in dry and moist concrete or Base materials/Ancillary materials
masonry. The SOUDAFIX VE400-SF product can also be used The declared product SOUDAFIX VE400-SF is delivered as a
for water-filled boreholes. The declared product SOUDAFIX two-component plastic cartridge and consists of a resin
VE400-SF has very good mechanical and thermal properties as component and a curing agent component in a 10:1 volume
well as very high chemical resistance. It can be used in ratio. The mixing ratio between the resin component and the
aggressive environments. The declared product SOUDAFIX curing agent component is set automatically as the product is
VE400-SF emits only a slight odour. pushed out of the cartridge. Curing begins immediately after the
components are mixed.
Sample applications
Suitable for securing façades, canopies, wooden structures,
metal structures, metal profiles, supports, beams, panels, 1) "This product/article/at least one partial article contains
railings, gratings, plumbing fixtures, pipes, cable trays, post- substances in the ECHA candidate list of substances of very
installed rebar connections (for renovations or reinforcement), high concern (SVHC) (10 June 2022) above a concentration of
etc. 0.1% by mass: no."
Technical Data
The following construction data are relevant for the declared
product SOUDAFIX VE400-SF as delivered: 2) "This product/article/at least one partial article contains other
Construction data CMR substances in categories 1A or 1B which are not on the
candidate list, exceeding 0.1 percentage by mass: no"
Name Value Unit
Density acc. to DIN 51757 for mixing the two
1.6 g/ml
components
Compressive strength acc. to DIN EN 196 Part 1 100.6N/mm² 3)"Biocide products were added to this construction product or
Flexural strength acc. to DIN EN 196 Part 1 14.7 N/mm² it has been treated with biocide products (this then concerns a
treated product as defined by the (EU) Regulation on Biocidal
Products No. 528/2012): no"
Storage:
Store in a cool, dry and dark place; storage temperature: +5°C
to +25°C
The product considered in this EPD contains individual
components in the following ranges:
Shelf life:
18 months in standard cartridge systems
18 months in foil tube cartridge systems
Resin component:
2 Environmental Product Declaration - SOUDAL N.V. - SOUDAFIX VE400-SF
Vinyl ester resin: 30 to 40% by weight
Other components: 10 to 35% by weight
Mineral fillers: 50 to 70% by weight
Reference service life
Other components: < 5% by weight The declared product SOUDAFIX VE400-SF may be exposed
to a wide range of environmental conditions during the use
phase. Its expected reference service life depends on the
specific installation situation and on the product's resulting
Curing agent component: exposure. The main factors influencing service life are weather
Dibenzoyl peroxide: 10 to 15% by weight conditions and mechanical and chemical stresses.
Mineral fillers: 40 to 60% by weight
LCA: Calculation rules
The precursor products are sourced from Germany, England
Declared Unit and France, Transport is mainly done by truck. Only the
The product declared is a two-component reaction resin mortar transport from England is done by rail. The following process
manufactured by SOUDAL N.V. with the product name diagrams illustrate the underlying production process.
SOUDAFIX VE400-SF. The declared unit is based on 1 kg
reaction resin product in the ratio at which the two components
must be mixed before use.
The mixing ratio between the resin component and the curing
agent component is 9:1 [m/m] (volume ratio 10:1). The
packaging is also included in the calculation at 0.3013 kg per 1
kg of reaction resin product. The declared unit data are
presented in the table below.
Declared unit data
Name Value Unit
Declared unit 1 kg
System boundary
Type of EPD: Cradle to factory gate with options. The following
information modules are defined as system boundaries in this
study: Figure 1 Information modules A 1 to A3 of the product
Production stage (A1- A3):
• A1, Raw material extraction,
• A2, Transport to the manufacturer,
• A3, Manufacturing.
End of life (C1- C4): Figure 2 Information modules A 1 to A3 of the packaging
C1, Deconstruction/demolition,
Geographic Representativeness
C2, Transport,
Land or region, in which the declared product system is
C3, Waste processing,
manufactured, used or handled at the end of the product´s
C4, Disposal.
lifespan: Germany
Reuse, recovery and recycling potential (D)
Comparability
To precisely determine the indicators and environmental
Basically, a comparison or an evaluation of EPD data is only
impacts of the declared unit, a total of 8 information modules
possible if all the data sets to be compared were created
are considered. The information modules A1 to A3 describe the
according to EN 15804 and the building context, respectively
material provision, the transport to the production site, as well
the product-specific characteristics of performance, are taken
as the production processes of the product itself.
into account.
LCA: Scenarios and additional technical information
Packaging per declared unit
Characteristic product properties of biogenic carbon
No renewable raw materials are used in the product or the Name Value Unit
packaging. The biogenic carbon value is therefore reported as Packaging PP 0.0318 kg
zero. Packaging PA6 0.2696 kg
3 Environmental Product Declaration - SOUDAL N.V. - SOUDAFIX VE400-SF
End of Life (C1-C4) Reuse, recovery and recycling potential (D), relevant
The product is demolished by using an electric chisel. The scenario specifications
electrical energy consumption for this tool is estimated at 0.05 The product has no reuse, recovery or recycling potential.
MJ for the declared unit. The power consumption is calculated Information module D is therefore declared and reported as
using a European energy mix. Construcion waste is transported zero.
200 km by truck to a waste treatment facility. At the waste Name Value Unit
treatment facility, the construction waste is shredded and the
Reuse, recovery and recycling potential 0 kg
disposed of in a landfill.
Name Value Unit
Collected as mixed construction waste 1 kg
Shredding 1 kg
Disposal in landfill 1 kg
4 Environmental Product Declaration - SOUDAL N.V. - SOUDAFIX VE400-SF
LCA: Results
DESCRIPTION OF THE SYSTEM BOUNDARY (X = INCLUDED IN LCA; MND = MODULE OR INDICATOR NOT DECLARED; MNR
= MODULE NOT RELEVANT)
Benefits and
Construction loads beyond
Product stage Use stage End of life stage
process stage the system
boundaries
la ire ta m w a Ry lp p u s tro p s n a rT g n iru tc a fu n a M e h t m o rf tro p s n a rTe tis e h t o t e ta g y lb m e s s A e s U e c n a n e tn ia M ria p e R tn e m e c a lp e R tn e m h s ib ru fe R y g re n e la n o ita re p Oe s u re ta w la n o ita re p Oe s u n o itc u rts n o c -e Dn o itilo m e d tro p s n a rT g n is s e c o rp e ts a W la s o p s iD -e s u e R-y re v o c e R-g n ilc y c e Rla itn e to p
A1 A2 A3 A4 A5 B1 B2 B3 B4 B5 B6 B7 C1 C2 C3 C4 D
X X X MND MND MND MND MNR MNR MNR MND MND X X X X X
RESULTS OF THE LCA - ENVIRONMENTAL IMPACT according to EN 15804+A2: 1 kg SOUDAFIX VE400-SF
Parameter Unit A1-A3 C1 C2 C3 C4 D
Global Warming Potential total (GWP-total) kg CO 2 eq 4.68E+00 5.12E-03 1.51E-02 2.6E-03 1.45E-02 0
Global Warming Potential fossil fuels (GWP-fossil) kg CO 2 eq 4.68E+00 5.12E-03 1.5E-02 2.59E-03 1.45E-02 0
Global Warming Potential biogenic (GWP-biogenic) kg CO 2 eq 0 0 0 0 0 0
Global Warming Potential luluc (GWP-luluc) kg CO 2 eq 8E-04 1.08E-06 8.28E-05 1.2E-05 2.67E-05 0
Depletion potential of the stratospheric ozone layer (ODP) kg CFC11 eq 6.24E-09 7.5E-14 8.9E-16 3.85E-15 3.4E-14 0
Acidification potential of land and water (AP) mol H+ eq 7.09E-03 1.12E-05 4.67E-05 1.34E-05 1.03E-04 0
Eutrophication potential aquatic freshwater (EP-freshwater) kg P eq 2.57E-05 1.49E-08 4.43E-08 7.43E-09 2.45E-08 0
Eutrophication potential aquatic marine (EP-marine) kg N eq 2.29E-03 2.52E-06 2.15E-05 6.11E-06 2.62E-05 0
Eutrophication potential terrestrial (EP-terrestrial) mol N eq 2.1E-02 2.65E-05 2.4E-04 6.74E-05 2.88E-04 0
Formation potential of tropospheric ozone photochemical oxidants kg NMVOC
6.57E-03 6.82E-06 4.22E-05 1.66E-05 7.97E-05 0
(POCP) eq
Abiotic depletion potential for non fossil resources (ADPE) kg Sb eq 1.14E-06 1.4E-09 1.24E-09 2.87E-09 1.48E-09 0
Abiotic depletion potential for fossil resources (ADPF) MJ 9.01E+01 9.29E-02 1.98E-01 5.06E-02 1.9E-01 0
m3 world eq
Water use (WDP) 1.49E-01 1.17E-03 1.33E-04 4.99E-04 1.59E-03 0
deprived
RESULTS OF THE LCA - INDICATORS TO DESCRIBE RESOURCE USE according to EN 15804+A2: 1 kg SOUDAFIX VE400-SF
Parameter Unit A1-A3 C1 C2 C3 C4 D
Renewable primary energy as energy carrier (PERE) MJ 1.17E+01 5.16E-02 1.13E-02 4.06E-03 2.85E-02 0
Renewable primary energy resources as material utilization
MJ 0 0 0 0 0 0
(PERM)
Total use of renewable primary energy resources (PERT) MJ 1.17E+01 5.16E-02 1.13E-02 4.06E-03 2.85E-02 0
Non renewable primary energy as energy carrier (PENRE) MJ 6.07E+01 9.3E-02 1.99E-01 5.07E-02 1.9E-01 0
Non renewable primary energy as material utilization (PENRM) MJ 2.95E+01 0 0 0 0 0
Total use of non renewable primary energy resources (PENRT) MJ 9.02E+01 9.3E-02 1.99E-01 5.07E-02 1.9E-01 0
Use of secondary material (SM) kg 0 0 0 0 0 0
Use of renewable secondary fuels (RSF) MJ 0 0 0 0 0 0
Use of non renewable secondary fuels (NRSF) MJ 0 0 0 0 0 0
Use of net fresh water (FW) m3 1.33E-02 4.92E-05 1.28E-05 1.42E-05 4.82E-05 0
RESULTS OF THE LCA – WASTE CATEGORIES AND OUTPUT FLOWS according to EN 15804+A2:
1 kg SOUDAFIX VE400-SF
Parameter Unit A1-A3 C1 C2 C3 C4 D
Hazardous waste disposed (HWD) kg 9.76E-09 8.04E-12 9.53E-13 6.34E-13 9.75E-12 0
Non hazardous waste disposed (NHWD) kg 8.53E-02 7E-05 2.85E-05 1.34E-05 9.71E-01 0
Radioactive waste disposed (RWD) kg 1.33E-03 1.49E-05 2.45E-07 6.68E-07 2.11E-06 0
Components for re-use (CRU) kg 0 0 0 0 0 0
Materials for recycling (MFR) kg 0 0 0 0 0 0
Materials for energy recovery (MER) kg 0 0 0 0 0 0
Exported electrical energy (EEE) MJ 0 0 0 0 0 0
Exported thermal energy (EET) MJ 0 0 0 0 0 0
RESULTS OF THE LCA – additional impact categories according to EN 15804+A2-optional:
1 kg SOUDAFIX VE400-SF
Parameter Unit A1-A3 C1 C2 C3 C4 D
Disease
Incidence of disease due to PM emissions (PM) ND ND ND ND ND ND
incidence
Human exposure efficiency relative to U235 (IR) kBq U235 eq ND ND ND ND ND ND
Comparative toxic unit for ecosystems (ETP-fw) CTUe ND ND ND ND ND ND
Comparative toxic unit for humans (carcinogenic) (HTP-c) CTUh ND ND ND ND ND ND
Comparative toxic unit for humans (noncarcinogenic) (HTP-nc) CTUh ND ND ND ND ND ND
5 Environmental Product Declaration - SOUDAL N.V. - SOUDAFIX VE400-SF
Soil quality index (SQP) SQP ND ND ND ND ND ND
The dataset "DE: Epoxy Resin, Source: Sphera, Reference year: 2021" was updated with reference to the previous EPD. As this
dataset has a strong influence on the overall calculation, the results are higher in comparison to the previous EPD from 2015.
References
Standards ETA-10/0167
European Technical Assessment.
DIN 51757
DIN 51757:2011-01 ETA-21/0170
Testing of mineral oils and related materials - Determination of European Technical Assessment.
density
ETA-12/0558
EN 196 European Technical Assessment.
DIN EN 196-1:2016-11
Test methods for cement - Part 1: Determination of strength IBU 2021
German version EN 196-1:2016 Institut Bauen und Umwelt e.V.: General guidance for the EPD
programme of the Institut Bauen und Umwelt e.V., Version 2.0,
EN 15804 Berlin: Institut Bauen und Umwelt e.V., 2021.
EN 15804:2019-04+A2, Sustainability of construction works - www.ibu-epd.com
Environmental Product Declarations - Core rules for the product
category of construction products. PCR PART A
Product Category Rules for Building-Related Products and
ISO 14025 Services - Calculation Rules for the Life Cycle Assessment and
DIN EN ISO 14025:2011-10, Environmental labels and requirements on the Project Report V2.1, Institut Bauen und
declarations - Type III environmental declarations - Principles Umwelt e.V., 11.2021.
and procedures.
PCR: Reaction resin products
ISO 14044 Guidance-Texts for Building-Related Products and Services.
DIN EN ISO 14044:2006-10, Environmental management - Life Part B: Requirements on the EPD for Reaction resin products,
cycle assessment - Requirements and guidelines. Version 1.3. Berlin: Institut Bauen und Umwelt e.V.
(Hrsg.),07.2014.
Further references Sphera
GaBi 10 Software: Life Cycle Assessment
Leinfelden-Echterdingen; Sphera Solution GmbH (Hrsg.).
ecoinvent 3.7.1 http://www.gabi-software.com/deutsch/index/
Background database: ecoinvent 3.7.1 (25/03/2022)
Zürich: ecoinvent (Ed.) .
http://www.ecoinvent.org
(25/03/2022) Regulation (EU) No. 305/2011 (CPR)
Regulation (EU) No. 528/2012 (Biocidal Product Regulation)
6 Environmental Product Declaration - SOUDAL N.V. - SOUDAFIX VE400-SF
Publisher
Institut Bauen und Umwelt e.V. +49 (0)30 3087748- 0
Hegelplatz 1 info@ibu-epd.com
10117 Berlin www.ibu-epd.com
Germany
Programme holder
Institut Bauen und Umwelt e.V. +49 (0)30 3087748- 0
Hegelplatz 1 info@ibu-epd.com
10117 Berlin www.ibu-epd.com
Germany
Author of the Life Cycle Assessment
FIT-Umwelttechnik GmbH 05362 72 69 474
Westerstr. 13 bertram@fit-umwelttechnik.de
38442 Wolfsburg www.fit-umwelttechnik.com
Germany
Owner of the Declaration
SOUDAL N.V. +32 014 42 42 31
Everdongenlaan 18-20 info@soudal.com
2300 Turnhout www.soudal.com
Belgium
7 Environmental Product Declaration - SOUDAL N.V. - SOUDAFIX VE400-SF
