ENVIRONMENTAL PRODUCT DECLARATION
as per ISO 14025 and EN 15804+A2
Owner of the Declaration Armacell International S.A.
Publisher Institut Bauen und Umwelt e.V. (IBU)
Programme holder Institut Bauen und Umwelt e.V. (IBU)
Declaration number EPD-ARM-20220389-IBA1-EN
Issue date 12.01.2024
Valid to 11.01.2029
ArmaPET® Eco50
Armacell
www.ibu-epd.com | https://epd-online.com
1. General Information
Armacell ArmaPET® Eco50
Programme holder Owner of the declaration
IBU – Institut Bauen und Umwelt e.V. Armacell International S.A.
Hegelplatz 1 Westside Village, rue Pafebruch 89B
10117 Berlin L-8308 Capellen - GD of Luxembourg
Germany Luxembourg
Declaration number Declared product / declared unit
EPD-ARM-20220389-IBA1-EN The declared product is ArmaPET® Eco50. The declared unit relates to 1
m³ of product, with an average density of 50 kg/m3. The packaging is also
included in the calculation. The declared unit is given in [m³].
This declaration is based on the product category rules: Scope:
Insulating materials made of foam plastics, 01.08.2021 This document relates to ArmaPET® Eco50. For the creation of the life
(PCR checked and approved by the SVR) cycle assessment, specific data was collected from the manufacturing
plant in Thimister-Clermont in Belgium of the Armacell Group, which
corresponds to the annual average and is based on data from 2022 (see
Issue date 3.8 allocation). The owner of the declaration is liable for the information
and evidence on which it is based; the IBU accepts no liability for
12.01.2024
manufacturer information, life cycle assessment data and evidence.
The owner of the declaration shall be liable for the underlying information
and evidence; the IBU shall not be liable with respect to manufacturer
Valid to
information, life cycle assessment data and evidences.
11.01.2029
The EPD was created according to the specifications of EN 15804+A2. In
the following, the standard will be simplified as EN 15804.
Verification
The standard EN 15804 serves as the core PCR
Independent verification of the declaration and data according to ISO
14025:2011
internally X externally
Dipl.-Ing. Hans Peters
(Chairman of Institut Bauen und Umwelt e.V.)
Florian Pronold Dr. Matthew Fishwick,
(Managing Director Institut Bauen und Umwelt e.V.) (Independent verifier)
1 Environmental Product Declaration - Armacell - ArmaPET® Eco50
2. Product
Name Value Unit
2.1 Product description/Product definition
Gross density acc. to EN 1602 50 kg/m3
ArmaPET® Eco50 is a low-density polyethylene terephthalate
(PET) foam, based on 100% recycled plastic bottles. Its long- Reaction to fire - EN 13501-1 E -
term stability of the insulation properties and the low thermal Compressive strength acc. to EN
CS(10\Y)150 N/mm2
conductivity secure lifetime insulation performance. The water 826
resistance and the closed-cell structure of the material ensure Calculation value for thermal
stable thermal conductivity even after many years of operation. conductivity acc. to EN 12667 <0,035 W/(mK)
These features also prevent moisture penetration, mildew and and EN 13164 Annex C
rot and therefore offer long-term corrosion protection and
Water vapour diffusion resistance
minimal maintenance requirements. >1000 -
factor acc. to EN 12086
Additionally, the material can be thermoformed into curved
Thermal conductivity acc. to EN
shapes, welded in pre-fabrication or on site, and is versatile for <0,030 W/(mK)
12667
use in almost any type of finishing options. Its thermoplastic
Dimensional Stability at 23°C;
nature also allows for full recyclability of the material after the
relative change in length/width ΔƐ ≤ ± 1 %
use phase.
EN1603
Thanks to Armacell's patented rPET technology, ArmaPET®
Eco50 is based on 100% recycled PET and is manufactured Dimensional Stability at 70°C ΔƐ ≤ 6 for thickness
according to an energy and resource optimised production and 90% RH; relative change in 20-40mm; ΔƐ ≤ 5 for %
process: with the re-use of waste material and no use of ozone- length/width/thickness EN1604 thickness 41-200mm
depleting hydrofluorocarbons (HFC) or chlorofluorcocarbons Dimensions: Thickness acc. to
T3
(CFC) blowing agents. EN823
For the placing of the product on the market in the European ± 8mm for boards ≤
Union/European Free Trade Association /EU/EFTA) (with the Dimension: width acc. to EN822 1500mm; ±10mm for
exception of Switzerland) the Regulation (EU) No. 305/2011 boards > 1500mm
(CPR) applies. The product needs a declaration of performance
± 8mm for boards ≤
taking into consideration ETA No. 21/0623; 26.10.2022;
Dimension: length acc. to EN822 1500mm; ±10mm for
"ArmaPET Eco50 - Factory-made products of extruded, foamed
boards > 1500mm
Polyethylene terephthalate (PET) for thermal and or acoustical
Squareness acc. to EN824 <5 mm/m
insulation" and the CE-marking.
For the application and use the respective national provisions Flatness acc. to EN825 <6 mm
apply. Long term water absorption by
immersion acc. to EN12087, WL(T)3
2.2 Application
method 2A
ArmaPET® Eco50 offers a solution for the (semi-) structural Deformation under specified
insulation of building envelopes, roofs, floors and internal compressive load and
partitions, in new building construction and the renovation of temperature condition acc. to DLT(2)5
older buildings. EN1605
Intended use, as specified in ETA No. 21/0623, is thermal
insulation in walls (including cellar walls), ceilings, floors, roofs, Performance data of the product in accordance with the
between rafters and timber work. The provisions made in the declaration of performance with respect to its essential
ETA are based on an assumed intended working life of 50 characteristics according to ETA No. 21/0623; 26.10.2022;
years for the insulation product. The indications given on the "ArmaPET Eco50 - Factory-made products of extruded, foamed
working life cannot be interpreted as a guarantee given by the Polyethylene terephthalate (PET) for thermal and or acoustical
producer, but are to be regarded only as a means for choosing insulation".
the right product in relation to the expected reasonable working
2.4 Delivery status
life of the works.
ArmaPET® Eco50 is supplied in boards. A flexible thickness
2.3 Technical Data range from 20 to 200 mm is available, with standard widths of
For further technical data consult the product datasheet 1000 or 1220 mm and length options between 500 and 3000
available on mm.
the website. Acoustic properties are not relevant for ArmaPET®
2.5 Base materials/Ancillary materials
Eco50.
Name Value Unit
Technical Data
Recycled PET 94,8 Gew.-%
Table in accordance with the Declaration of Performance
Fillers and modifiers 1,2 Gew.-%
Blowing agent 4 Gew.-%
ArmaPET® Eco50 is a low density, closed-cell foam, produced
based on 100% recycled PET. Mechanically recycled PET is
mixed in a molten state with additives that ensure a stable
foaming process. These include nucleating agents, viscosity
modifiers, foam stabilisers and a physical blowing agent.
The nucleating agent determines the foam's cell size
distribution. The viscosity modifier ensures sufficient melt
strength for foaming by increasing the molecular weight of the
2 Environmental Product Declaration - Armacell - ArmaPET® Eco50
PET, broadening its molecular weight distribution and
introducing long-chain branches. The physical blowing agent
expands the foam to achieve the required density range.
Eventually, the additional modifiers and stabilisers support the
process stability and help to avoid cell coalescence.
This product contains substances listed in the candidate list
(date: 14.06.2021) exceeding 0.1 percentage by mass: no.
This product contains other CMR substances in categories 1A
or 1B which are not on the candidate list, exceeding 0.1
percentage by mass: no.
Figure: Illustration of the ArmaPET Eco50 Production Process
Biocide products were added to this construction product or it
2.7 Environment and health during manufacturing
has been treated with biocide products (this then concerns a
All our plants employ environmental monitoring systems, and
treated product as defined by the (EU) Ordinance on Biocide
we exchange ideas and best practices via the internal
Products No. 528/2012): no.
communications network. We collect key performance
2.6 Manufacture indicators on energy use, CO 2 emissions, water consumption
ArmaPET Eco50 foam boards are manufactured based on and waste management in order to evaluate and continually
mechanically recycled PET, applying the patented technology improve our sustainability performance. 13 of Armacell's plants
of Armacell. This method is based on reprocessing post- are environmentally certified acc. to ISO 14001, and the energy
consumer PET waste to produce recycled flakes, after management systems at our German facilities in Münster and
separation of the polymer from contaminants. It includes sorting Friesenhofen are certified to ISO 50001 as well. Environmental
and separating of waste, washing it to remove any dirt and management at Armacell is implemented in line with the
contaminants, and further grinding, crushing and sorting carried 'Environment' pillar of the World-Class Armacell Mindset
out by Armacell's suppliers. The recycled product is compliant Manufacturing program. This program maintains consistency in
with the predefined specification of Armacell and is supplied in standards and sustains the implementation of improved
the form of flakes and granules. processes. It is based on the systematic identification of losses
At Armacell, the flakes are processed into granules by melt- and non-value-added tasks at Armacell's multi-technology sites.
extrusion. The granulation process includes pre-drying the
2.8 Product processing/Installation
flakes to avoid hydrolysis in the extrusion process. The pre-
dryed flakes are fed into an extruder where the material is ArmaPET® Eco50 can be used on its own and/or as part of a
molten and homogenized. A vacuum extraction section is used system, depending on the application. It can be handled and
to remove volatile contaminants from the melt. After final installed without any special precautions for personal and
filtration the material is granulated by underwater cutting environmental protection. Further advice on handling and
followed by crystallization of the obtained rPET granules. installation can be found in the related product literature
provided by the manufacturer.
Obtained recycled PET granules are further processed into
2.9 Packaging
foam through foaming extrusion, in the presence of halogen-
free supercritical fluid used as a physical blowing agent. Further ArmaPET® Eco50 boards are stacked on reusable wooden
components of the foam include additives for foam nucleation, pallets for transport and storage. These pallets comply with the
cell stabilization and melt modification. The patented method of ISPM15 regulation. All pallets are protected in a way that
rPET treatment and modification during melt processing allows prevents damage at the corners of the boards, and plastic
Armacell to overcome the main disadvantage of mechanical wrapping ensures protection from moisture and dirt. The
recycling – a decline in the product quality – and to upgrade the polyethylene- and carton-based packaging elements are
quality despite the thermal degradation, photo-oxidation and recyclable and (actually) recycled in the countries having a
mechanical stresses. return system.
Another component of the formulation is 'PET Agglomerate',
2.10 Condition of use
which is obtained from reclaimed PET foam.
When the products are used for the purpose for which they are
The primary source of agglomerate is the PET dust generated
intended, there are no changes in the materialE composition
by the lateral and surface grinding operations in the
during use, except in the event of extraordinary impacts (see
downstream of the foam extrusion process (Eco50 internal
2.14).
loop). Another source of agglomerate, is PET foam which is
diverted from the waste stream of other PET foam products at
2.11 Environment and health during use
Armacell. All reclaimed foam cut-offs are crushed and
ArmaPET® Eco50 does not contain any Substances of Very
compacted in a first step. In the second step, the pre-
High Concern (SVHC) or any compounds that are persistent,
compacted particles are mixed with reclaimed PET dust and
bioaccumulative and/or toxic (PBT). No environmental damage
partially molten by shear forces and formed into agglomerate
or health risks are to be expected during normal conditions of
through a template. The extruded foamed PET boards with
homogeneous and closed-cell structure are calibrated, edge cut use. ArmaPET® Eco50 has been assessed in terms of the
and surface grinded to obtain the final product with the required emission of regulated dangerous substances from construction
dimensions and surface planarity. products into indoor air (according to EN16516) and the results
confirm that no substances are emitted in quantities above the
European limits.
2.12 Reference service life
ArmaPET® materials are long-lasting products with a designed
lifetime of 25 to 50 years. The service life is practically only
restricted by the lifetime in the application. The insulation
3 Environmental Product Declaration - Armacell - ArmaPET® Eco50
performance is maintained throughout the entire service life, Mechanical destruction
thanks to the low water absorption, closed-cell cellular structure ArmaPET® Eco50 is designed for load bearing and non-load
and the high solubility of a foaming agent in the PET matrix. bearing (semi‑) structural insulation applications and has a
The insulation performance can only be compromised by compression strength of >150 kPa when used as a standalone
extraordinary impacts and damage during construction. material. It can withstand certain mechanical impacts during
Description of the influences on the ageing of the product when handling and storage without significant damage.
applied in accordance with the rules of technology.
2.14 Re-use phase
In the non-contaminated form, the product is fully recyclable by
2.13 Extraordinary effects a mechanical recycling scheme for PET. It could be shredded
Fire into smaller pieces and reprocessed to granules using
According to the European fire classification system, extrusion and reused as tertiary recycled pellets in the non-food
ArmaPET® Eco50 is classified as combustible insulation contact applications (e.g. for foaming processes, fibres
material of Euroclass E, tested as per EN ISO 11 925-2 by spinning, injection moulding, etc.).
means of the ignitability test. For classes A2 to D, additional In case of severe contamination and problems with separation,
classification using the SBI test procedure (Single Burning Item the product could be recycled via chemical recycling with bis(2-
test) in accordance with EN 13823 is required. hydroxyethyl) terephthalate (BHET) or dimethyl terephthalate
(DMT) or monomers purified therephthalic acid and mono-
Fire protection
ethylene glycol (PTA and MEG, respectively) recovery,
Name Value
depending on the recycling method (glycolysis or hydrolysis).
Building material class acc. to EN 13501-1 E
2.15 Disposal
Dispose of the materials according to local regulations.
Water
Regulated by the European Waste Catalogue: Waste code 07
ArmaPET® Eco50 is chemically neutral, not water soluble, and
420 (other non-hazardous plastic waste). Note: Please observe
if used for the intended purpose does not release any water-
Commission Decision 2001/118/EC.
soluble substances that might pollute groundwater, rivers or
oceans. Water or water vapour has virtually no impact on the
2.16 Further information
thermal conductivity. For water exposure tests please revise the
Further Information on ArmaPET Eco50 can be found on the
Table of point 2.3 and for water leakages - point 7.2.
manufacturer's website www.armacell-core-foams.com
3. LCA: Calculation rules
provision of materials, the transport to the production site, as
3.1 Declared Unit well as the production processes of the product itself.
The declared product is an ArmaPET Eco50. The declared unit
relates to 1 m³ of product. The packaging with 3,039 kg is also
included in the calculation. The following table shows the data 3.3 Estimates and assumptions
of the declared unit. For the rPET flakes, no specific data could be provided by the
supplier. In the background databases only rPET granulate is
Declared unit
available. For this reason, the background data for rPET pellets
Name Value Unit
without the influence of the electrical energy of the granulation,
Declared unit 1 m3 were used for the calculation of the rPET flakes in module A1.
Average density 50 kg/m³ This assumption is important for the calculation of the EPD as a
whole, in order to avoid double counting, because in module A3
Weight 50 kg
a specific granulation at Armacell is calculated for this material.
3.2 System boundary 3.4 Cut-off criteria
The type of the EPD is from the cradle to the factory gate with The cut-off criterion according to EN 15804+A2 is applied. All
options, modules C1-C4 and module D. The following energy and mass inputs were taken into account.
information modules are defined as system limits in this study:
3.5 Background data
A1–A5 Product development: The background data b ase of the LCA for Experts and
A1 – Production of raw materials ecoinvent 3.9.1 databases, to which this study alsorefers, is
A2 – Transport to the manufacturer documented under the following link.(Sphera)
A3 – Production
A4 – Transport from the factory gate to the construction site 3.6 Data quality
A5 – Installation of the products in the building For the preparation of the life cycle assessment, specific data
was collected the Thimister-Clermont plant in Belgium, from the
End of life stage (C1- C4): company Armacell International S.A. and from the year 2022.
C1, deconstruction/demolition, The background data from the LCA for Experts and ecoinvent
C2, transport, 3.9.1 databases are from the year 2023 and therefore of high
C3, waste treatment , relevance.
C4, disposal. The masses of the different components of the insulation
boards are from the composition data.
Reuse, recovery and recycling potential (D) The data quality is rated as adequate.
3.7 Period under review
In order to precisely record the indicators and environmental
impacts of the declared unit, a total of 8 information modules The life cycle inventory analysis data provided by the
are considered. The information modules A1 to A3 describe the manufacturer is from 2022 and corresponds to
4 Environmental Product Declaration - Armacell - ArmaPET® Eco50
the annual average. with a total mass of all the manufactured foams equal to
8.770.995,60 kg, out of which 367.683 kg accounts for
3.8 Geographic Representativeness ArmaPET Eco50. The data linked to energy and water
Land or region, in which the declared product system is consumptions are collected collectively at the plant level and
manufactured, used or handled at the end of the product´s are allocated to the processes used in the Eco50 production
lifespan: Europe based on individual allocation factors for the processes. The
energy consumption data are collected separately for the
extrusion, granulation, and warehousing operations and are
3.9 Allocation
allocated to Eco50 production based on those allocation
The data presented in this EPD for ArmaPET Eco50 are
factors. The total waste, measured separately on a yearly basis
collected based on the yearly manufacturing output of
for all the produced items is allocated. Based on the total
Armacell's plant in Thimister-Clermont/ Belgium. Currently, this
allocation factor for Eco50.
is the only location manufacturing Eco50. In general, the split
between all the manufactured items covers: 3.10 Comparability
Basically, a comparison or an evaluation of EPD data is only
possible if all the data sets to be compared were created
according to EN 15804 and the building context, respectively
the product-specific characteristics of performance, are taken
into account.
The database referred to in this study is LCA for
Experts by Sphera and ecoinvent 3.9.1.
4. LCA: Scenarios and additional technical information
weight of the floor. Due to the different methods, auxiliary parts
Characteristic product properties biogenic carbon (screws, adhesive) are not included in the model.
No renewable raw materials are used in the product.
Name Value Unit
Therefore, the biogenic carbon is shown as zero. The following
Material loss 1.5 kg
raw materials contain biogenic carbon in the packaging.
Plastic Packaging Waste 0,075 kg
Information on describing the biogenic Carbon Content at
Cardboard Waste 0,510 kg
factory gate
Wood Waste 2,42 kg
Name ValueUnit
Biogenic carbon content in accompanying kg End of life (C1-C4)
1.27
packaging C
The product is demolished with an electric saw.
Note: 1 kg of biogenic carbon is equivalent to 44/12 kg of CO2 The electrical energy consumption for the tool is a value of 0.6
MJ is assumed for the declared unit. The electricity
consumption is calculated with one euro electricity mix. The
rubble is transported per truck 50 km to the waste treatment
plant.
Transport to the building site (A4)
Name Value Unit
The transport model considers a construction site in Western
Europe (Germany, Benelux). The scenario for the distribution Collected separately waste type waste type 50 kg
phase assumes a standard distance of 500 km. Recycling 24.2 kg
The transported quantity corresponds to the transport of the Energy recovery 2.6 kg
products and their packaging to the construction site.
Name Value Unit Reuse, recovery and/or recycling potentials (D), relevant
scenario information
Transport distance 500 km
Module D shows the utilization of the waste from the specified
Gross density of products transported 53.009 kg/m3
unit. It is assumed that 90 % is recycled and 10 % is thermally
utilized. Module D does not take into account the 23,067 kg of
Installation into the building (A5)
PET foam recovered from the other lines.
The application phase considers:
-Product losses Name Value Unit
-Waste treatment (product losses, product packaging). ArmaPET Eco 50 24,2 kg
Products are installed on the floor or on the wall manually.
The recycling potential of the ArmaEco 50 (45kg) is credited in
There are different ways to install the product, it could be fixed
this module. A collection rate of 90% is assumed.
with adhesive, mechanical fixing, etc. The most representative
application is just laid out on the floor and kept in place by the
5 Environmental Product Declaration - Armacell - ArmaPET® Eco50
5. LCA: Results
DESCRIPTION OF THE SYSTEM BOUNDARY (X = INCLUDED IN LCA; ND = MODULE OR INDICATOR NOT DECLARED; MNR =
MODULE NOT RELEVANT)
Benefits and
Construction loads beyond
Product stage Use stage End of life stage
process stage the system
boundaries
la ire ta m w a Ry lp p u s tro p s n a rT g n iru tc a fu n a M e h t m o rf tro p s n a rTe tis e h t o t e ta g y lb m e s s A e s U e c n a n e tn ia M ria p e R tn e m e c a lp e R tn e m h s ib ru fe R y g re n e la n o ita re p Oe s u re ta w la n o ita re p Oe s u n o itc u rts n o c -e Dn o itilo m e d tro p s n a rT g n is s e c o rp e ts a W la s o p s iD -e s u e R-y re v o c e R-g n ilc y c e Rla itn e to p
A1 A2 A3 A4 A5 B1 B2 B3 B4 B5 B6 B7 C1 C2 C3 C4 D
X X X X X MND MND MNR MNR MNR MND MND X X X X X
RESULTS OF THE LCA - ENVIRONMENTAL IMPACT according to EN 15804+A2: 1 m³ ArmaPET Eco 50
Parameter Unit A1-A3 A4 A5 C1 C2 C3 C4 D
GWP-total kg CO 2 eq 3.48E+01 1.98E+00 6.22E+00 5.44E-02 1.88E-01 1.63E+00 5.96E+00 -2.76E+01
GWP-fossil kg CO 2 eq 3.97E+01 1.96E+00 8.41E-01 5.44E-02 1.86E-01 1.63E+00 5.96E+00 -2.76E+01
GWP-biogenic kg CO 2 eq -5.38E+00 0 5.38E+00 0 0 0 0 0
GWP-luluc kg CO 2 eq 5.2E-01 1.8E-02 -1.54E-04 5.84E-06 1.7E-03 1.15E-03 7.48E-06 -3.2E-02
ODP kg CFC11 eq 1.06E-06 1.7E-13 -1.32E-11 9.92E-13 1.6E-14 2.75E-11 3.81E-13 -9.3E-07
AP mol H+ eq 1.28E-01 2.13E-03 -1.84E-03 1.15E-04 2.2E-04 3.85E-03 5.69E-04 -1.03E-01
EP-freshwater kg P eq 1.17E-02 7.07E-06 -1.29E-06 2.01E-07 6.68E-07 5.97E-06 9.02E-08 -1.04E-02
EP-marine kg N eq 4.94E-02 7.19E-04 -6.34E-04 2.75E-05 7.48E-05 1.07E-03 1.61E-04 -3.13E-02
EP-terrestrial mol N eq 3.58E-01 8.51E-03 -5.39E-03 2.87E-04 9.04E-04 1.14E-02 2.74E-03 -2.53E-01
kg NMVOC
POCP 7.32E-01 1.86E-03 -1.84E-03 7.33E-05 1.89E-04 2.87E-03 4.5E-04 -9.2E-02
eq
ADPE kg Sb eq 1.93E-04 1.25E-07 -7.74E-08 8.34E-09 1.18E-08 3.71E-07 3.56E-09 -1.64E-04
ADPF MJ 1.03E+03 2.64E+01 -5.38E+01 1.13E+00 2.49E+00 3.37E+01 9.64E-01 -4.73E+02
m3 world eq
WDP 8.99E+00 2.23E-02 7.3E-01 1.2E-02 2.11E-03 3.55E-01 5.3E-01 -9.66E+00
deprived
GWP = Global warming potential; ODP = Depletion potential of the stratospheric ozone layer; AP = Acidification potential of land and water; EP =
Eutrophication potential; POCP = Formation potential of tropospheric ozone photochemical oxidants; ADPE = Abiotic depletion potential for non-fossil
resources; ADPF = Abiotic depletion potential for fossil resources; WDP = Water (user) deprivation potential)
RESULTS OF THE LCA - INDICATORS TO DESCRIBE RESOURCE USE according to EN 15804+A2: 1 m³ ArmaPET Eco 50
Parameter Unit A1-A3 A4 A5 C1 C2 C3 C4 D
PERE MJ 3.75E+02 1.87E+00 -3.85E+00 6.76E-01 1.76E-01 1.89E+01 2.45E-01 -5.86E+01
PERM MJ 7.64E+00 0 0 0 0 0 0 0
PERT MJ 3.75E+02 1.87E+00 -3.85E+00 6.76E-01 1.76E-01 1.89E+01 2.45E-01 -5.86E+01
PENRE MJ 1.03E+03 2.64E+01 -5.38E+01 1.13E+00 2.5E+00 3.37E+01 9.64E-01 -4.73E+02
PENRM MJ 4.4E+00 0 0 0 0 0 0 0
PENRT MJ 1.03E+03 2.64E+01 -5.38E+01 1.13E+00 2.5E+00 3.37E+01 9.64E-01 -4.73E+02
SM kg 2.31E+01 0 0 0 0 0 0 0
RSF MJ 0 0 0 0 0 0 0 0
NRSF MJ 0 0 0 0 0 0 0 0
FW m3 3.12E-01 2.06E-03 1.28E-02 5.46E-04 1.94E-04 1.58E-02 1.25E-02 -2.29E-01
PERE = Use of renewable primary energy excluding renewable primary energy resources used as raw materials; PERM = Use of renewable primary
energy resources used as raw materials; PERT = Total use of renewable primary energy resources; PENRE = Use of non-renewable primary energy
excluding non-renewable primary energy resources used as raw materials; PENRM = Use of non-renewable primary energy resources used as raw
materials; PENRT = Total use of non-renewable primary energy resources; SM = Use of secondary material; RSF = Use of renewable secondary fuels;
NRSF = Use of non-renewable secondary fuels; FW = Use of net fresh water
RESULTS OF THE LCA – WASTE CATEGORIES AND OUTPUT FLOWS according to EN 15804+A2:
1 m³ ArmaPET Eco 50
Parameter Unit A1-A3 A4 A5 C1 C2 C3 C4 D
HWD kg 1.01E-06 9.78E-11 -6.12E-09 -8.86E-11 9.24E-12 -2.44E-09 2.21E-11 -1.75E-09
NHWD kg 2.51E-01 3.81E-03 1.04E-01 8.29E-04 3.6E-04 2.35E-02 2.82E-02 -1.64E-02
RWD kg 9.39E-02 3.42E-05 -4.72E-03 1.8E-04 3.23E-06 4.99E-03 5.81E-05 -2.57E-03
CRU kg 0 0 0 0 0 0 0 0
MFR kg 0 0 0 0 0 0 0 0
MER kg 0 0 0 0 0 0 0 0
EEE MJ 0 0 0 0 0 0 0 0
EET MJ 0 0 0 0 0 0 0 0
HWD = Hazardous waste disposed; NHWD = Non-hazardous waste disposed; RWD = Radioactive waste disposed; CRU = Components for re-use;
MFR = Materials for recycling; MER = Materials for energy recovery; EEE = Exported electrical energy; EET = Exported thermal energy
6 Environmental Product Declaration - Armacell - ArmaPET® Eco50
RESULTS OF THE LCA – additional impact categories according to EN 15804+A2-optional:
1 m³ ArmaPET Eco 50
Parameter Unit A1-A3 A4 A5 C1 C2 C3 C4 D
Disease
PM ND ND ND ND ND ND ND ND
incidence
IR kBq U235 eq ND ND ND ND ND ND ND ND
ETP-fw CTUe ND ND ND ND ND ND ND ND
HTP-c CTUh ND ND ND ND ND ND ND ND
HTP-nc CTUh ND ND ND ND ND ND ND ND
SQP SQP ND ND ND ND ND ND ND ND
PM = Potential incidence of disease due to PM emissions; IR = Potential Human exposure efficiency relative to U235; ETP-fw = Potential comparative
Toxic Unit for ecosystems; HTP-c = Potential comparative Toxic Unit for humans (cancerogenic); HTP-nc = Potential comparative Toxic Unit for humans
(not cancerogenic); SQP = Potential soil quality index
Disclaimer 2 – for the indicators 'abiotic depletion potential for non-fossil resources', 'abiotic depletion potential
for fossil resources', 'water (user) deprivation potential, deprivation-weighted water consumption', 'potentialcomparative toxic unit for
ecosystems', 'potential comparative toxic unit for humans – cancerogenic', 'Potentialcomparative toxic unit for humans - not
cancerogenic', 'potential soil quality index'.The results of this environmental impact indicator shall be used with care as theuncertainties
on these results are high as there is limited experience with the indicator
6. LCA: Interpretation
The dominance analysis shows that the main causes of
environmental impacts and indicators are to be found in
information module A1. This can be seen in the total global
warming potential for material supply with approx. 27%, related
to all information modules and a saving of 35% from information
module D.v
Diagram: Dominance analysis A1 –Raw material acquisition
If we look at the exact composition of the ArmaPET Eco 50, it
becomes clear that the main contributor to the global warming
potential is the rPET flakes with approximately. 78%.
Diagram: Dominance analysis - Modules A1 to D
If we look at the material supply for the product and the
packaging in detail, it becomes clear that two raw materials
contribute decisively to the respective environmental impacts
and indicators.
The material supply of the ArmaPET Eco 50 generates approx.
84% of the total global warm-ing potential and approx. 95% of
the total non-renewable primary energy in the information
module A1. For wood, it is approx. 13% of the total global
warming potential and approx. 3% of the total non-renewable
primary energy in the information module A1.
Diagram: Dominance analysis A1 -Raw material acquisition of
ArmaPET Eco50
In the information module A3 it is clear that the main cause of
environmental impact and indicators is in the production of
ArmaPET Eco 50, with a global warming potential of 98%.
7 Environmental Product Declaration - Armacell - ArmaPET® Eco50
Diagram: Dominance analysis A3 – Production
7. Requisite evidence
7.1 VOC emissions
The product has been tested for determination 7.2 Leaching performance
of the volatile organic compound emissions according to
EN16516:2017 'Construction Measurement of leaching performance has
products: Assessment of release of dangerous substances - been indicatively tested based on DIN EN 13468: 'Thermal
Determination of insulating products
emissions into indoor air'. The test has been performed by for building equipment and industrial installations -
Servaco/ Normec Determination of trace
Product Testing (Wetteren, Belgium) on June 11th, 2021, quantities of water soluble chloride, fluoride, silicate, and
and the results are covered by the test report SPT2021-R084. sodium ions and
The data are expressed for Floor and Wall application. pH', at Armacell. Test temperature was 100 °C, with a
leaching time of 0,5 h. The results on water leachable ions
AgBB overview of results (28 days [µg/m³])
specified in
Name Value Unit
mg/kg are summarized in the table.
TVOC (C6 - C16) Floor application 27 μg/m3
Sum SVOC (C16 - C22) Floor application <5 μg/m3
R (dimensionless) Floor application 3 -
VOC without NIK Floor application 27 μg/m3
Carcinogenic Substances Floor application <1 μg/m3
TVOC (C6 - C16) Wall application 69 μg/m3
Sum SVOC (C16 - C22) Wall application <5 μg/m3
R (dimensionless) Wall application 0,0007 -
VOC without NIK Wall application 69 μg/m3
Carcinogenic Substances Wall application <1 μg/m3
8. References
CML 2001 April. 2015 applications - Determination of squareness.
Indicators for
environmental impacts DIN EN 825
Leiden: Universität Leiden
http://cml.leiden.edu/software/data-cmlia.html#downloads DIN EN 825:2013-10-23: Thermal insulating products for
(30.11.2021) building applications - Determination of flatness.
ECHA-List DIN EN 826
Candidate List of substances of very high concern for DIN EN 826:2013: Thermal insulating products for building
Authorisation, applications - Determination of
https://echa.europa.eu/candidate-list-table (2021) compression behaviour.
CPR DIN EN 1603
Regulation (EC) No DIN EN 1603:2013-05: Thermal insulating products for building
305/2011, Construction Products Regulation applications - Determination of
dimensional stability under constant normal laboratory
DIN EN 824 conditions (23 °C/ 50 % relative humidity).
DIN EN 824:2013-05:Thermal insulating products for building
8 Environmental Product Declaration - Armacell - ArmaPET® Eco50
DIN EN 1604 apparent density.
DIN EN 1604:2013-05:Thermal insulating products for building
applications - Determination of EN1609
dimensional stability under specified temperature and humidity EN1609:2013: Thermal insulating products for building
conditions. applications - Determination of
short-term water absorption by partial immersion.
DIN EN 1605
DIN EN 1605:2013-05:Thermal insulating products for building EN 11925
applications - Determination of EN ISO 11925-2:2020: Reaction to fire tests - Ignitability of
deformation under specified compressive load and temperature products subjected to direct impingement of flame - Part 2:
conditions. Single-flame source test.
DIN EN 1606 EN 12086
DIN EN 1606: 2013: Thermal insulating products for building DIN EN 12086:2013-06:Thermal insulating products for building
applications - Determination of applications - Determination of water vapour transmission
compressive creep. properties.
DIN EN 1607 DIN EN 12087
DIN EN 1607:2013: Thermal insulating products for building DIN EN 12087:2013-06:Thermal insulating products for building
applications - Determination of applications - Determination of long term water absorption by
tensile strength perpendicular to faces. immersion.
DIN EN 12091 EN 12088
DIN EN 12091:2013: Thermal insulating products for building EN 12088:2013: Thermal insulating products for building
applications - Determination of applications - Determination of
freeze-thaw resistance. long-term water absorption by diffusion.
DIN EN 12667 EN 12089
DIN EN 12667:2001: Thermal performance of building materials EN 12089:2013: Thermal insulating products for building
and products - Determination of thermal resistance by means of applications - Determination of
guarded hot plate and heat flow meter methods - Products of bending behaviour.
high and medium thermal resistance.
EN 13164
DIN EN 13468 EN 13164:2012 Annex C: Thermal insulation products for
DIN EN 13468: 2001 Thermal insulating products for building buildings - Factory made extruded
equipment and industrial installations - Determination of trace polystyrene foam (XPS) products – Specification.
quantities of water-soluble chloride, fluoride, silicate, and
sodium ions and pH. EN 13501
EN13501-1: 2018 : Fire classification of construction products
DIN EN 15801 and building elements - Part 1: Classification using data from
DIN EN 15801:2010: Conservation of cultural property - Test reaction to fire tests.
methods - Determination of water absorption by capillarity.
EN13823
DIN EN 29052 EN13823:2020: Reaction to fire tests for building products -
DIN EN 29052-1:1991: Acoustics; determination of dynamic Building products excluding floorings exposed to the thermal
stiffness - Part 1: Materials used attack by a single burning item.
under floating floors in dwellings.
EN 15804
EAD EN 15804:2012+A2:2019 + AC:2021, Sustainability of
European Assessment Document no. 040179-00-1201, March construction works - Environmental Product Declarations - Core
2016, 'Factory-made products of extruded, foamed rules for the product category of construction
Polyethylene terephthalate (PET) for thermal and/or acoustical products.
insulation'.
EN 16516
ETA EN 16516:2017 Construction products: Assessment of release
of dangerous substances -
European Technical Assessment No. 21/0623; 26.10.2022; Determination of emissions into indoor air.
"ArmaPET Eco50 - Factory-made products of extruded, foamed
Polyethylene terephthalate (PET) for thermal and or acoustical EN 16535
insulation". EN ISO 16535:
2019: Thermal insulating products for building applications -
ecoinvent 3.9.1 Determination of long-term water absorption by immersion.
Background database: ecoinvent 3.9.1
Zürich: ecoinvent European Waste Catalogue
http://www.ecoinvent.org 2001/118/EC: Commission Decision of 16 January 2001
(23.05.2023). amending Decision 2000/532/EC as regards the list of wastes
(Text with EEA relevance) (notified under document number
EN 1602 C(2001) 108)
EN 1602:2013: Thermal insulating products for building https://op.europa.eu/en/publication-detail/-
applications - Determination of the /publication/429c2c5d-9be3-11e4-872e-
9 Environmental Product Declaration - Armacell - ArmaPET® Eco50
01aa75ed71a1/language-en InternatIonal Standard for Phyto-sanitary Measures 15:
Regulation of wood packaging material in international trade,
IBU 2021 Adopted 2018; published 2019.
General Instructions for the EPD programme of Institut Bauen
und Umwelt e.V. Version 2.0, PCR Part A
Berlin: Institut Bauen und Umwelt e.V., 2021www.ibu-epd.de Product category rules for construction products and services -
Calculation rules for the eco-balance and requirements for the
ISO 1402 background report V1.3, Institut Bauen und Umwelt
DIN EN /ISO14025:2011-10/, Environmental labels and e.V.,08.2022.
declarations - Type III environmental
declarations - Principles and procedures. Product category rules for construction products – Part B
Insulating materials made of foam plastics, 01.08.2021.
ISO 14001
ISO 14001:2015: Environmental management systems - Servaco/ Normec Product Testing
Requirements with guidance for use. https://normecservaco.com/en/dienst/normec-product-testing/
ISO 14044 Sphera
DIN EN ISO14044:2006-10: Environmental management - Life LCA for Experts Software: Ganzheitliche Bilanzierung
cycle assessment - Requirements and guidelines. Leinfelden-Echterdingen; Sphera
Solution GmbH
ISO 29767 http://www.gabi-software.com/deutsch/index/
ISO 29767:2019: Thermal insulating products for building (23.05.2023).
applications - Determination of
short-term water absorption by partial immersion. REACH
Regulation (EC) No 1907/2006, Regulation concerning the
ISO 50001 Registration,
ISO 50001:2018: Energy management systems - Requirements Evaluation, Authorisation and Restriction of Chemicals
with guidance for use. (REACH)
with further amendments of 14.06.2021.
ISPM 15
10 Environmental Product Declaration - Armacell - ArmaPET® Eco50
Publisher
Institut Bauen und Umwelt e.V. +49 (0)30 3087748- 0
Hegelplatz 1 info@ibu-epd.com
10117 Berlin www.ibu-epd.com
Germany
Programme holder
Institut Bauen und Umwelt e.V. +49 (0)30 3087748- 0
Hegelplatz 1 info@ibu-epd.com
10117 Berlin www.ibu-epd.com
Germany
Author of the Life Cycle Assessment
FIT-Umwelttechnik GmbH 05362 72 69 474
Westerstr. 13 bertram@fit-umwelttechnik.de
38442 Wolfsburg www.fit-umwelttechnik.com
Germany
Owner of the Declaration
Armacell International S.A. +49-251-7603227
Westside Village, rue Pafebruch 89B heribert.quante@armacell.com
L-8308 Capellen - GD of Luxembourg www.armacell.com
Luxembourg
11 Environmental Product Declaration - Armacell - ArmaPET® Eco50
