ENVIRONMENTAL PRODUCT DECLARATION
as per ISO 14025 and EN 15804+A2
Owner of the Declaration Grundfos Holding A/S
Publisher Institut Bauen und Umwelt e.V. (IBU)
Programme holder Institut Bauen und Umwelt e.V. (IBU)
Declaration number EPD-GRU-20230079-CBC1-EN
Issue date 21.11.2023
Valid to 20.11.2028
MAGNA3 65-80/100/120 (Cast Iron)
Grundfos Holding A/S
www.ibu-epd.com | https://epd-online.com
General Information
Grundfos Holding A/S MAGNA3 65-80/100/120 (Cast Iron)
Programme holder Owner of the declaration
IBU – Institut Bauen und Umwelt e.V. Grundfos Holding A/S
Hegelplatz 1 Poul Due Jensens Vej 7
10117 Berlin 8850 Bjerringbro
Germany Denmark
Declaration number Declared product / declared unit
EPD-GRU-20230079-CBC1-EN 1 PCS. of MAGNA3 65-80/100/120 (Cast Iron)
This declaration is based on the product category rules: Scope:
Pumps for liquids and liquids with solids, 01.08.2021 The declaration applies to 1 piece of MAGNA3 (Cast Iron) pump.
(PCR checked and approved by the SVR)
Issue date The product is produced in Wahlstedt, Germany, and the life cycle
assessment is based on data collected at the production site.
21.11.2023
Valid to
Production has been modeled using annual production data from 2021.
20.11.2028
The declaration covers three different types of the MAGNA3 65- product
(80/100/120).
The owner of the declaration shall be liable for the underlying information
and evidence; the IBU shall not be liable with respect to manufacturer
information, life cycle assessment data and evidences.
The EPD was created according to the specifications of EN 15804+A2. In
the following, the standard will be simplified as EN 15804.
Verification
Dipl.-Ing. Hans Peters
(Chairman of Institut Bauen und Umwelt e.V.) The standard EN 15804 serves as the core PCR
Independent verification of the declaration and data according to ISO
14025:2011
internally X externally
Florian Pronold Mrs Kim Allbury,
(Managing Director Institut Bauen und Umwelt e.V.) (Independent verifier)
1 Environmental Product Declaration - Grundfos Holding A/S - MAGNA3 65-80/100/120 (Cast Iron)
Product
Product description/Product definition
The Grundfos MAGNA3
circulator pumps are designed for circulating liquids in heating The products are also
systems, air identical in terms of packaging, distribution, reference service
conditioning and cooling systems and domestic hot water life and
systems. However, the end-of-life treatment.
pump range can also be used in ground source heat pump
systems and solar
heating systems.
The only thing that
differentiates the products from each other is the software
which controls how
the pump operates in the system in which it is installed, making
them fit for
different applications. Hence, all life cycle modules are
identical, except use
The MAGNA3 pump is a stage module B6, which will change, as the applied scenarios
centrifugal pump powered by an electrical motor. It has a high- for electricity
performance consumption changes. For the placing on the market in the
neodymium magnet rotor which increases motor efficiency and European Union/European Free Trade Association (EU/EFTA)
an insulation shell (with
to reduce heat loss from the cast iron pump housing with the exception of Switzerland) the following legal
threaded connections. provisions as well as the corresponding harmonised
norms based on these provisions apply:
Machinery
Directive (2006/42/EC)
Standard used: EN
The declaration covers 809:1998 + A1:2009.
three types of the MAGNA3 pump. They are grouped as shown
below. The group
reference in the technical data and scenarios refers also to
these.
Radio Equipment
Directive (2014/53/EU)
GROUP 1 - MAGNA3 65-80
Standards used:
EN 60335-1:2012/AC:2014 + A11:2014, EN 60335-2-51:2003 +
A1:2008 + A2:2012,
GROUP 2 - MAGNA3 65-100 EN 62233:2008.
GROUP 3 - MAGNA3 65-120
EN 55014-1:2006
+ A1:2009 + A2:2011, EN 55014-1:2017, EN 61000-6-2:2005,
These are all the same EN 61000-3-2:2014, EN
physical products and 100 % identical in terms of design, 61000-3-3:2013, ETSI EN 301 489-1 V2.2.0, ETSI EN 301 489-
dimensions and 17 V3.2.0. ETSI EN 300 328 V2.1.1
materials as well as supply chain and manufacturing processes,
i.e., all cradle
to gate processes (A1-A3).
Electromagnetic
Compatibility (EMC) Directive (2014/30/EU)
2 Environmental Product Declaration - Grundfos Holding A/S - MAGNA3 65-80/100/120 (Cast Iron)
are not harmonized in accordance with the CPR.
Standards used: EN
55014-1:2017, EN 55014-2:2015, Application
For the
application and use the respective national
provisions
EN apply.
61000-3-2:2014/2019, EN 61000-6-2:2008/2019,
EN 61000-3-3:2013
A1:2019
The pump is
designed for circulating liquids in the
following
RoHS Directive systems:
2011/65/EU and 2015/863//EU
·
Standard: EN heating systems
50581:2012.
·
domestic hot-water systems
Ecodesign ·
Directive (2009/125/EC) air-conditioning and cooling systems
Commission Regulation ·
(EC) No: 641/2009 and ground-source heat-pump systems
Commission ·
Regulation (EU) 622/2012 solar-heating systems
Standards used: The pump is
EN 16297-1:2012, EN 16297-2:2012, EN 16297-3:2012. suitable for thin, clean, non-aggressive and non-explosive
liquids, not
containing solid particles or fibres that may attack the pump
mechanically or
chemically. In heating systems, the water must meet the
requirements of accepted
standards on water quality
in heating systems. The pumps are also suitable for domestic
The CE-marking hot-water systems
takes into account the proof of conformity with the respective
Technical Data
harmonized norms
based on the legal provisions above. The performance
data of the product according to the harmonized norms, based
on the
harmonization provisions above apply.
The relevant
MAGNA3 pumps technical specifications according to the PCR Part B are given
3 Environmental Product Declaration - Grundfos Holding A/S - MAGNA3 65-80/100/120 (Cast Iron)
in REACH
the table below.
This product/article/at
Characteristics least one partial article contains
that are the same for all product groups are only given once.
Others are given
individually for all three groups.
substances
Constructional data
listed in the ECHA candidate list (date:
Name ValueUnit
Frequency 50 Hz
Voltage 230 V
Energy Efficiency Index Gr.1 0,18 10.06.2022)
exceeding 0.1 percentage by mass: no
Energy Efficiency Index Gr.2 0,17
Energy Efficiency Index Gr.3 0,17
Flow range Gr. 1 (max) 37,5 m3/h
Flow range Gr. 2 (max) 40,0 m3/h
Flow range Gr. 3 (max) 42,50m3/h
Head max. Gr.1 8 m
Head max. Gr.2 10 m The Wahlstedt
Head max. Gr.3 12 m production has been assessed and certified as meeting the
Power input Gr. 1 Average (from load profile requirements in ISO 14001,
0,197 kW
describing use) ISO 50001, ISO 45001 and ISO 9001.
Power input Gr. 2 Average (from load profile
0,249 kW Reference service life
describing use)
No use stage
Power input Gr. 3 Average (from load profile 0,320 kW scenario which refers to the lifetime of the product is declared.
describing use) However, to
Nominal capacity Gr.1 0,461 kW facilitate building calculations, an estimated RSL of 10 years
Nominal capacity Gr. 2 0,599 kW can be used.
This is an EU consensus-based estimation, referenced on page
Nominal capacity Gr.3 0,75 kW
37 in Appendix 7: Lot
Performance 11 – Circulators in Buildings, prepared by AEA Energy &
data of the product according to the Environment for
the European Commission in the context of the Eco Design
Directive:
harmonized
standards, based on provisions for harmonization.
Base materials/Ancillary materials
Name Value Unit
Aluminium 13 %
Cast iron 53 % There is no
definitive information on the average circulator life available,
Ceramics 0,3 %
there is consensus
Copper 3 %
within the industry that it is at least 12 years. However, this is
Electronics 0,2 %
complicated by
Magnet Nd 1 % many factors, including many being scrapped prematurely
Paper 0,5 % when e.g. the
PCB 4 % boiler they are connected to is replaced.
Plastics 0,3 %
Plastics, foam 1 %
Plastics GF 5 %
Rubber 0,2 %
Stainless steel 4 %
Steel 8 %
From the
Cardboard 8 %
estimated stock (140Mpa) and annual sales (14Mpa), the
Plastic film 0,1 % average lifetime of
TOTAL 100 % the circulator is taken as 10 years for the purposes of this study.
4 Environmental Product Declaration - Grundfos Holding A/S - MAGNA3 65-80/100/120 (Cast Iron)
B6 is declared per year as required by the PCR Part B.
The RSL of the
declared product is not directly influencing the results in this
study, as no
declared use stage scenario is dependent on the RSL; The use
stage sub-module
LCA: Calculation rules
Declared Unit
The declared
unit is 1 piece (pcs.) of MAGNA3 (Cast Iron) pump.
Declared unit
Name Value Unit
Declared unit 1 pce.
Mass reference 23.9 kg/pce
Conversion factor [Mass/Declared Unit] 23.9
The product
For IBU core EPDs (where clause 3.6 is part of the EPD): for
stage is included in the study, and according to EN 15804 the
average EPDs, an estimate of the robustness of the LCA
system
values must be made, e.g. concerning the variability of the
boundary with nature is set to include those processes that
production process, geographical representativeness and the
provide the
influence of background data and preliminary products
material and energy inputs into the system and the following
compared to the environmental impacts caused by the actual
manufacturing,
production.
transport up to the factory gate as well as the processing any
waste arising
System boundary from those processes.
This EPD is
Cradle-To-Grave. The system boundaries
Wastes and
losses are included in the modules where they occur according
to the polluter
of the EPD
pays principle and the modular approach of EN 15804.
follow the modular approach in EN 15804. By decision no.
20170712-n of
the SVR, the modules B3, B4 and B5 are by default declared
as
"MNR" (module not relevant).
The
product includes:
The product
·
stage (A1-A3) comprises raw
A1 Extraction and processing of raw materials;
material extraction and processing, transport processes as well
as the
manufacturing process. The final production and assembly of
the MAGNA3 pump
·
takes place at a Grundfos manufacturing site in Germany.
A1 Reuse of products or materials from a previous product
However, the full
system;
supply-chain leading to the finished product at the gate is rather
complex and
includes a large amount of raw materials, components and
semi-finished parts
·
which comes from both external suppliers as well as other
A1 Processing of secondary materials;
Grundfos production
facilities.
5 Environmental Product Declaration - Grundfos Holding A/S - MAGNA3 65-80/100/120 (Cast Iron)
· is produced from the incineration are considered as closed-loop
A1 Generation of electricity, steam and heat from primary within A1-A3, as
energy resources, described in PCR Part A, 5.5.1. The input of biogenic carbon
also including their extraction, refining and transport; from the
production of packaging material is inventoried in A3. As
required by PCR
Part A, the corresponding end-of-life module of the packaging
· material, A5, is also declared and the emissions of biogenic
A1 Energy recovery and other recovery processes from carbon are
secondary fuels; inventoried.
·
A2 Transportation up to the factory gate and internal transport;
The
· construction process stage (A4-A5) includes:
A3 Production of ancillary materials or pre products;
A4:
·
A3 Manufacturing of products and coproducts;
·
Transportation from factory gate to distribution center:
·
A3 Manufacturing of packaging;
·
Consumption of electricity, thermal energy and water at
· distribution center;
A1-A3 processing up to the end-of-waste state or disposal of
final residues.
·
Transportation from distribution center to construction site;
For secondary
material inputs, the system boundary to the previous system
(providing the
secondary material) is set where outputs reach the end-of- ·
waste state. The Wastage during distribution.
recycling of secondary material into new raw materials is
included in the
system boundary of this study. Waste
A5:
materials from
production processes that are recycled without any modification ·
of the material's Installation process;
inherent characteristics are modelled as closed-loop within A1-
A3. This is done
up to the input mass flow that was used during production.
·
Transport of packaging waste to treatment site;
·
Waste treatment of packaging.
Waste for
incineration arising in the product stage is accounted for in the
module where
the waste is produced. The environmental loads from the The packaging
incineration process material does not reach the end of waste state but is
are declared in the module where it occurs and the electricity incinerated as waste.
and heat which According to European statistics, the average R1 value of
6 Environmental Product Declaration - Grundfos Holding A/S - MAGNA3 65-80/100/120 (Cast Iron)
incineration plants B4 and B5
is > 0.6. Therefore, it is assumed are by default declared as "MNR" (module
that packaging not relevant).
material is treated thermally in an incineration plant with R1 > The modules include the provision and transport of all
0.6. The materials, products and
loads from the combustion process of packaging are declared related energy and water use, as well as waste processing up
in module A5 and to the
the resulting energy benefits in module end-of-waste state or disposal of final residues during the use
stage. They
also include all impacts and
D, as required
by the PCR Part A, 5.5.2.
aspects related
to the losses during the use stage (i.e. production, transport,
and waste
processing and disposal of the lost products and materials).
Use stage
(B1-B7):
Generally, the
geographical coverage of the datasets used matches the actual
processes taking
place. Meaning, that when modelling taking place in Grundfos
Bjerringbro,
The use stage, the Danish electricity grid mix is used in the model and thermal
related to the building fabric includes: energy
from natural gas. These are generally of very high quality with
very good
technological, temporal and geographical representativeness.
·
B1, use or application of the installed product;
·
B2, maintenance.
Contributions
to operational energy use during the use stage (B6) come from
the electricity
The use stage consumption of the product. The annual electricity consumption
related to the operation of the building is calculated by
multiplying the average power input, which is based on a
defined load profile,
with the annual running hours. For use stage (B6) European
includes: Average
electricity grid mix has been used. These values are declared in
the scenarios
section.
·
B6, operational energy use;
·
B7, operational water use.
The End-of-Life
stage (C1-C4) includes all
activities from when the product reaches the end of its service
In this study, life and no
all use stage modules are assessed, though B1, B2 and B7 are longer provides any functionality and until all materials and
assessed to be components are
zero. By decision no. 20170712-n of the SVR, the modules B3, processed for
7 Environmental Product Declaration - Grundfos Holding A/S - MAGNA3 65-80/100/120 (Cast Iron)
An
overall collection rate of 90 % has been assumed.
reuse/recycling
or disposed of.
Materials from
which energy is recovered in an incineration process with an
R1-value above 0.60
According to EN are in this study included with the environmental burdens from
15804 and the PCR Part A, the end-of-life stage the incineration
includes: process inventoried in C3, the recovered energy is declared as
exported energy
in C3
·
C1 deconstruction of the product from the
and the energy
benefits are declared in D. This procedure is according to the
PCR Part A,
· 5.5.6. C3 includes the mechanical separation of the product
building, including initial on-site sorting of the followed by a
series of sorting steps. Metal fractions are recycled and
plastics, cardboard
and electronics are assumed incinerated with energy recovery.
· The residual
materials; fractions are landfilled and declared in C4.
· The specific
C2 transportation of the discarded product to a recycling site amounts are shown in the scenarios section.
and
transportation of waste to final disposal;
·
C3 waste processing, collection of waste fractions from the
deconstruction and Beyond system
waste processing of material flows intended for reuse, recycling boundary (D): According to EN
and energy 15804 module D includes the reuse, recovery and/or recycling
recovery; potentials,
expressed as net impacts and benefits. Any declared benefits
and loads from net
·
C4 waste disposal including physical pretreatment and
management of the flows leaving
disposal site. the product system that have not been allocated as co-products
and that have
passed the end-of-waste state are included in module D.
At the end of life,
the MAGNA3 pump is manually disassembled from the piping
system in which it has
been installed. The definition of the applied end-of-life scenario
in this EPD
follows the requirements in the
Contributions
to module D comes from waste incineration processes in A5
and C3 as well as
PCR Part A, 6.2 regarding complex products, with a material recycling in C3. The specific fractions and net flows are
combination shown in the
of recycling, thermal waste treatment and landfilling. 100 % of scenarios section.
the material is
considered in the end of life scenario as required by the PCR.
8 Environmental Product Declaration - Grundfos Holding A/S - MAGNA3 65-80/100/120 (Cast Iron)
Basically, a comparison or an evaluation of EPD data is only
possible if all the data sets to be compared were created
according to EN 15804 and the building context, respectively
the product-specific characteristics of performance, are taken
Comparability into account. Software and
databases used: GaBi ts
Basically, a
comparison or an evaluation of EPD data is only possible if all
the data sets
to be compared were created according to EN
15804 and the building context, respectively the product-
specific
characteristics of performance, are taken into account. 9.2.1.68
(database schema 8007) Ecoinvent v3.5..
Geographic Representativeness
Land or region, in which the declared product system is
manufactured, used or handled at the end of the product´s
lifespan: Germany
Comparability
LCA: Scenarios and additional technical information
Name Value Unit
Characteristic product properties of biogenic carbon
Litres of fuel 0,0332 l/100km
The biogenic
Transport distance 2003 km
carbon content quantifies the amount of biogenic carbon in a
construction Capacity utilisation (including empty runs) 85 %
product leaving the factory gate, and it will be separately Gross density of products transported 460 kg/m3
declared for the
Wastage during distribution 0,02 %
product and for any accompanying packaging, as required from
the PCR Part A. Installation into the building (A5)
The Carbon content of Cardboard and Paper is assumed to
Name ValueUnit
0.46 kg C. Overall,
Packaging waste for incineration (LDPE film) 0,031 kg
there is an amount of 9 weight-% Carbon in the product leaving
the factory gate Packaging waste for incineration 1,95 kg
and has to be considered (Paper/Cardboard)
An
estimated RSL of 10 years can be used to facilitate building
calculations. This
is an EU consensus-based estimation, referenced in Appendix
Information on describing the biogenic Carbon Content at 7: Lot 11 –
factory gate Circulators in Buildings, prepared by AEA Energy &
Environment for the
Name ValueUnit
European Commission in the context of the Eco Design
Biogenic carbon content in accompanying kg
0.74 Directive.
packaging C
Note: 1 kg of biogenic carbon is equivalent to 44/12 kg of CO2
The following technical scenario information is required for the
Reference service life
declared modules and optional for non-declared modules.
Name Value Unit
Modules for which no information is declared can be deleted;
additional information can also be listed if necessary. Life Span according to the manufacturer 10 a
Operational energy use (B6)
The following technical information is a basis for the declared
modules or can be used for developing specific scenarios in the Name Value Unit
context of a building assessment if modules are not declared Electricity consumption Group 1 985 kWh/a
(MND).
Electricity consumption Group 2 1245 kWh/a
Electricity consumption Group 3 1600 kWh/a
A5 is not declared including the disposal of the packaging
material on the construction site, the amounts of packaging Average power input, Group 1 0,197 kW
materials included in the LCA calculations must be declared as Average power input, Group 2 0,249 kW
technical scenario information for Module A5. Average power input, Group 3 0,32 kW
Running hours (all groups) 5.000 h/a
Transport from the gate to the site (A4) End of life (C1-C4)
9 Environmental Product Declaration - Grundfos Holding A/S - MAGNA3 65-80/100/120 (Cast Iron)
Name ValueUnit Reuse, recovery and/or recycling potentials (D), relevant
Collected as mixed construction waste 21,94 kg scenario information
Transportation distance (C2) 500 km Name Value Unit
Aluminium for recycling 2,79 kg A5, incineration w/energy recov. (LDPE foil) 4,37 MJ
Steel for recycling 12,7 kg A5, incineration w/energy recov.
7,91 MJ
Copper for recycling 0,60 kg (Paper/Cardboard)
Stainless steel for recycling 0,84 kg C3, steel for recycling (net amounts) -1,28 kg
Paper/Cardboard for for incineration w/energy C3, stainless steel for recycling (net amounts) 0,52 kg
1,95 kg
recovery C3, aluminium for recycling (net amounts) -0,383 kg
Plastics for incineration w/energy 1,39 kg C3, copper for recycling (net amounts) 0,258 kg
Electronics for incineration w/energy 0,81 kg C3, plastics for incineration, w/ energy recov. 1,39 kg
Landfilling 2,81 kg C3, electronics for incineration, w/ energy recov. 0,81 kg
10 Environmental Product Declaration - Grundfos Holding A/S - MAGNA3 65-80/100/120 (Cast Iron)
LCA: Results
Characterization
model: EN 15804 - 2012+A2 - 2019, PEF. By Decision no. 20170712-n of the
IBU SVR, the modules B3, B4, B5 are marked as MNR (module not relevant) as
default. The LCA results in module B6 are given on a period of one year,
according to PCR Part B. To obtain the results from module B6 over the
entire life cycle, the LCA results of module B6 must be multiplied by the
estimated RSL of 10 years. The indicator results for module B6 are
declared for Group 1. B6 indicator results for other groups can be derived by
multiplying the B6 indicator results with the following factors:
Group 2 PN6/10: 1,265
Group 3 PN6/10: 1,626
Group 2 PN16: 1,29
Group 3 PN16: 1,55
DESCRIPTION OF THE SYSTEM BOUNDARY (X = INCLUDED IN LCA; ND = MODULE OR INDICATOR NOT DECLARED; MNR =
MODULE NOT RELEVANT)
Benefits and
Construction loads beyond
Product stage Use stage End of life stage
process stage the system
boundaries
la ire ta m w a Ry lp p u s tro p s n a rT g n iru tc a fu n a M e h t m o rf tro p s n a rTe tis e h t o t e ta g y lb m e s s A e s U e c n a n e tn ia M ria p e R tn e m e c a lp e R tn e m h s ib ru fe R y g re n e la n o ita re p Oe s u re ta w la n o ita re p Oe s u n o itc u rts n o c -e Dn o itilo m e d tro p s n a rT g n is s e c o rp e ts a W la s o p s iD -e s u e R-y re v o c e R-g n ilc y c e Rla itn e to p
A1 A2 A3 A4 A5 B1 B2 B3 B4 B5 B6 B7 C1 C2 C3 C4 D
X X X X X MND MND MNR MNR MNR X MND X X X X X
RESULTS OF THE LCA - ENVIRONMENTAL IMPACT according to EN 15804+A2: 1PCS of MAGNA3 65-80/100/120 (Cast Iron)
Parameter Unit A1 A2 A3 A4 A5 B6 C1 C2 C3 C4 D
GWP-total kg CO 2 eq 1.07E+02 1.46E+00 8.1E-01 1.49E+00 2.86E+00 3.98E+02 0 6.11E-01 6.65E+00 1.43E-01 -3.4E-01
GWP-fossil kg CO 2 eq 1.06E+02 1.45E+00 4.05E+00 1.48E+00 1.53E-01 3.97E+02 0 6.07E-01 6.64E+00 1.47E-01 -3.34E-01
GWP-
biogenic kg CO 2 eq 4.63E-01 -1.98E-03 -3.28E+00 -3.02E-03 2.7E+00 1.32E+00 0 -1.02E-03 6.57E-03 -4.43E-03 -2.68E-03
GWP-luluc kg CO 2 eq 1.82E-01 1.05E-02 3.66E-02 1.18E-02 9.69E-05 5.75E-01 0 4.93E-03 3.27E-03 1.29E-04 -3.03E-03
kg CFC11
ODP 9.52E-08 2.53E-16 4.07E-09 1.99E-11 5.23E-16 8.72E-12 0 1.12E-16 4.92E-14 3.31E-16 -7.6E-13
eq
AP mol H+ eq 5.65E-01 1.08E-02 1.7E-02 8.64E-03 8.22E-04 8.75E-01 0 3.58E-03 5.67E-03 4.57E-04 -1.35E-02
EP-
kg P eq 1.63E-03 3.99E-06 6.44E-05 4.77E-06 1.2E-07 1.06E-03 0 1.86E-06 8.65E-06 1.61E-05 -4.47E-06
freshwater
EP-marine kg N eq 7.27E-02 3.76E-03 3.3E-03 4.12E-03 3E-04 1.94E-01 0 1.73E-03 1.37E-03 1.37E-03 -5.12E-04
EP-terrestrial mol N eq 7.64E-01 4.16E-02 3.3E-02 4.56E-02 3.73E-03 2.04E+00 0 1.91E-02 1.53E-02 1.16E-03 -5.09E-03
kg NMVOC
POCP 2.26E-01 8.64E-03 9.46E-03 7.85E-03 7.83E-04 5.33E-01 0 3.28E-03 3.74E-03 3.39E-04 -1.74E-03
eq
ADPE kg Sb eq 5.89E-03 1.09E-07 5.96E-05 1.31E-06 8.71E-09 1.15E-04 0 4.93E-08 6.48E-07 9.95E-09 -7.2E-04
ADPF MJ 1.45E+03 1.92E+01 5.62E+01 2E+01 9.85E-01 6.97E+03 0 8.13E+00 4.01E+01 2.11E+00 -2.05E+01
m3 world eq
WDP 2.61E+01 1.29E-02 2.36E-01 2.07E-02 3.52E-01 8.64E+01 0 5.94E-03 9.34E-01 -1.63E-03 -4.92E-01
deprived
GWP = Global warming potential; ODP = Depletion potential of the stratospheric ozone layer; AP = Acidification potential of land and water; EP =
Eutrophication potential; POCP = Formation potential of tropospheric ozone photochemical oxidants; ADPE = Abiotic depletion potential for non-fossil
resources; ADPF = Abiotic depletion potential for fossil resources; WDP = Water (user) deprivation potential)
RESULTS OF THE LCA - INDICATORS TO DESCRIBE RESOURCE USE according to EN 15804+A2: 1PCS of MAGNA3 65-
80/100/120 (Cast Iron)
Parameter Unit A1 A2 A3 A4 A5 B6 C1 C2 C3 C4 D
PERE MJ 3.99E+02 1.01E+00 5.11E+01 1.25E+00 1.7E-01 3.09E+03 0 4.7E-01 1.74E+01 1.48E-01 4.06E+00
PERM MJ 0 0 0 0 -2.58E+01 0 0 0 -1.82E+00 0 0
11 Environmental Product Declaration - Grundfos Holding A/S - MAGNA3 65-80/100/120 (Cast Iron)
PERT MJ 3.99E+02 1.01E+00 5.11E+01 1.25E+00 1.7E-01 3.09E+03 0 4.7E-01 1.74E+01 1.48E-01 4.06E+00
PENRE MJ 1.45E+03 1.93E+01 5.62E+01 2E+01 9.86E-01 6.97E+03 0 8.16E+00 4.01E+01 2.11E+00 -2.04E+01
PENRM MJ 0 0 0 0 -6.9E-01 0 0 0 -2.39E+00 0 0
PENRT MJ 1.45E+03 1.93E+01 5.62E+01 2E+01 9.86E-01 6.97E+03 0 8.16E+00 4.01E+01 2.11E+00 -2.04E+01
SM kg 1.8E+01 0 2.31E-01 3.65E-03 0 0 0 0 0 0 0
RSF MJ 1.46E-23 0 0 2.91E-27 0 0 0 0 0 0 0
NRSF MJ 1.71E-22 0 0 3.42E-26 0 0 0 0 0 0 0
FW m3 8.16E-01 1.18E-03 2.57E-02 1.52E-03 8.29E-03 3.57E+00 0 5.48E-04 3.05E-02 2.68E-05 2.39E-02
PERE = Use of renewable primary energy excluding renewable primary energy resources used as raw materials; PERM = Use of renewable primary
energy resources used as raw materials; PERT = Total use of renewable primary energy resources; PENRE = Use of non-renewable primary energy
excluding non-renewable primary energy resources used as raw materials; PENRM = Use of non-renewable primary energy resources used as raw
materials; PENRT = Total use of non-renewable primary energy resources; SM = Use of secondary material; RSF = Use of renewable secondary fuels;
NRSF = Use of non-renewable secondary fuels; FW = Use of net fresh water
RESULTS OF THE LCA – WASTE CATEGORIES AND OUTPUT FLOWS according to EN 15804+A2:
1PCS of MAGNA3 65-80/100/120 (Cast Iron)
Parameter Unit A1 A2 A3 A4 A5 B6 C1 C2 C3 C4 D
HWD kg 3.3E-04 8.05E-07 1.22E-04 9.86E-07 5.11E-09 2.89E-06 0 3.78E-07 2.01E-08 8.46E-09 -3.25E-04
NHWD kg 4.29E+00 2.95E-03 2.91E-01 4.23E-03 9.43E-02 4.95E+00 0 1.29E-03 6.44E-01 2.42E+00 1.53E+00
RWD kg 6.21E-02 3.41E-05 1.55E-03 5.38E-05 4.74E-05 1.06E+00 0 1.5E-05 5.94E-03 2.53E-05 -1.71E-03
CRU kg 0 0 0 0 0 0 0 0 0 0 0
MFR kg 0 0 0 0 0 0 0 0 1.69E+01 0 0
MER kg 0 0 0 0 0 0 0 0 0 0 0
EEE MJ 0 0 0 0 4.37E+00 0 0 0 7.41E+00 0 0
EET MJ 0 0 0 0 7.91E+00 0 0 0 1.34E+01 0 0
HWD = Hazardous waste disposed; NHWD = Non-hazardous waste disposed; RWD = Radioactive waste disposed; CRU = Components for re-use;
MFR = Materials for recycling; MER = Materials for energy recovery; EEE = Exported electrical energy; EET = Exported thermal energy
RESULTS OF THE LCA – additional impact categories according to EN 15804+A2-optional:
1PCS of MAGNA3 65-80/100/120 (Cast Iron)
Parameter Unit A1 A2 A3 A4 A5 B6 C1 C2 C3 C4 D
Disease
PM 6.93E-06 1.28E-07 2.37E-07 5.13E-08 4.65E-09 7.34E-06 0 2.1E-08 4.79E-08 4.66E-09 -2.96E-07
incidence
IR kBq U235 eq 6.82E+00 5.03E-03 2.44E-01 7.53E-03 7.3E-03 1.74E+02 0 2.22E-03 9.74E-01 3.59E-03 -1.46E-01
ETP-fw CTUe 8.45E+02 1.43E+01 1.82E+01 1.46E+01 4.97E-01 2.98E+03 0 6.09E+00 1.75E+01 1.49E+00 -7.65E+00
HTP-c CTUh 1.62E-06 2.93E-10 6.46E-07 7.58E-10 2.44E-11 8.24E-08 0 1.26E-10 5.29E-10 8.53E-11 -6.76E-08
HTP-nc CTUh 2.5E-06 1.6E-08 5.68E-08 1.77E-08 1.15E-09 3.03E-06 0 7.22E-09 2.13E-08 7.44E-09 -5.99E-09
SQP SQP 4.14E+02 6.09E+00 9.71E+01 6.91E+00 2.68E-01 2.22E+03 0 2.85E+00 1.26E+01 1.53E-01 -1.71E+01
PM = Potential incidence of disease due to PM emissions; IR = Potential Human exposure efficiency relative to U235; ETP-fw = Potential comparative
Toxic Unit for ecosystems; HTP-c = Potential comparative Toxic Unit for humans (cancerogenic); HTP-nc = Potential comparative Toxic Unit for humans
(not cancerogenic); SQP = Potential soil quality index
Disclaimer
1 – for the indicator 'Potential Human exposure efficiency relative to U235'.
This impact category deals mainly with the eventual impact of low-dose ionizing
radiation on human health of the nuclear fuel cycle. It does not consider
effects due to possible nuclear accidents, occupational exposure or
radioactive waste disposal in underground facilities. Potential ionizing
radiation from the soil, radon and from some construction materials is
also not measured by this indicator.
Disclaimer 2 – for the
indicators 'abiotic depletion potential for non-fossil resources', 'abiotic
depletion potential for fossil resources', 'water (user) deprivation potential,
deprivation-weighted water consumption', 'potential comparative toxic unit for
ecosystems', 'potential comparative toxic unit for humans – cancerogenic',
'Potential comparative toxic unit for humans - not cancerogenic', 'potential
soil quality index'. The results of this environmental impact indicator shall
be used with care as the uncertainties on these results are high as there is
limited experience with the indicator.
12 Environmental Product Declaration - Grundfos Holding A/S - MAGNA3 65-80/100/120 (Cast Iron)
Disclaimer 3: JRC
Technical Reports, Version 2, 2018 Page 6, for the
indicator "EP-freshwater". This indicator has been calculated as 'kg
P eq' as required in the characterization model EUTREND model, Struijs et al.,
2009b, as implemented in ReCiPe;
References
Standards
PARLIAMENT AND
OF THE COUNCIL of 26 February
Machinery 2014 on the
Directive harmonistion of the laws of the Member
DIRECTIVE 2006/42/EC States relating
OF THE EUROPEAN to electromagnetic compatibility
PARLIAMENT AND
OF THE COUNCIL of 17 May
Ecodesign
2006 on Directive
machinery
DIRECTIVE
2009/125/EC OF THE EUROPEAN
Radio Equipment PARLIAMENT AND
Directive OF THE COUNCIL of 21 October
DIRECTIVE 2009
2014/53/EU OF THE EUROPEAN PARLIAMENT AND OF THE establishing a framework for the setting of
COUNCIL of 16 April 2014 on
the harmonisation of the laws of the Member States relating to
the making
available on the market of ecodesign
requirements for energy-related products
radio equipment
EC 641/2009
Electromagnetic
Compatibility (EMC) Directive COMMISSION
REGULATION (EC) No 641/2009 of 22 July 2009 implementing
Directive 2005/32/EC
of the European Parliament and of the Council with regard to
DIRECTIVE ecodesign
2014/30/EU OF THE EUROPEAN requirements for glandless standalone circulators and
13 Environmental Product Declaration - Grundfos Holding A/S - MAGNA3 65-80/100/120 (Cast Iron)
glandless circulators integrated Directive 2011/65/EU of the European
in
Parliament and
products of the Council as regards the list of
restricted
substances
EC 622/2012
COMMISSION
REGULATION (EU) No 622/2012 of 11 July 2012 amending ETSI EN 301
Regulation (EC) No 489-1
641/2009 with regard to ecodesign requirements for glandless
standalone
circulators and glandless circulators integrated in products
ETSI EN 301
489-1 V2.2.0, Electromagnetic Compatibility (EMC) standard for
radio equipment
and services; Part 1: Common technical requirements
DIRECTIVE
2011/65/EU
ETSI EN 301
DIRECTIVE 489-17
2011/65/EU OF THE EUROPEAN
ETSI EN 301
PARLIAMENT AND 489-17 V3.2.0, Electromagnetic Compatibility (EMC) standard
OF THE COUNCIL of 8 June 2011 for radio equipment
and services; Part 17: Specific conditions for Broadband Data
Transmission
Systems
on the
restriction of the use of certain hazardous
substances in
electrical and electronic equipment
DIRECTIVE
2015/863/EU ETSI EN 300 328
V2.1.1
DIRECTIVE
2015/863/EU of 31 March 2015 amending ETSI EN 300 328
V2.1.1, Wideband transmission systems; Data transmission
equipment operating in
the 2,4 GHz ISM band and using wide band modulation
Annex II to techniques
14 Environmental Product Declaration - Grundfos Holding A/S - MAGNA3 65-80/100/120 (Cast Iron)
EN 50581:2012,
Technical documentation for the
EN 809
assessment of
electrical and electronic products with
EN 809:1998-10
+ A1:2009, Pumps and pump units for
respect to the
restriction of hazardous substances
liquids -
Common safety requirements
EN 60335-1
EN 55014-1
EN
60335-1:2012/A11:2014/A13:2017, Household
EN
55014-1:2017, Electromagnetic compatibility – Requirements
for household and similar
appliances, electric tools and similar apparatus – Part 1: electrical appliances – Safety – Part 1:General requirements
Emission
EN 60335-2-51
EN 55014-2
EN
EN 60335-2-51:2003-03 + A1:2008 + A2:2012, Household and
55014-2:2015, Electromagnetic compatibility – similar electrical
appliances – Safety –Part 2-51: Particular requirements for
stationary
circulation pumps for heating and service water installations
Requirements
for household appliances, electric tools
and similar
apparatus – Part 2: Immunity – Product
EN 61000-3-2
family standard
(CISPR 14-2:2015) EN
61000-3-2:2014/2019, Electromagnetic compatibility (EMC) –
Part 3-2: Limits –
Limits for harmonic current emissions (equipment input current
=16 A per phase)
EN 50581:2012
15 Environmental Product Declaration - Grundfos Holding A/S - MAGNA3 65-80/100/120 (Cast Iron)
EN 61000-3-3 EN 16297-2:2012-10,
Pumps – Rotodynamic pumps –Glandless circulators – Part 2:
Calculation of
energy efficiency index (EEI) for standalone circulators
EN
61000-3-3:2013-08/ A1:2019, Electromagnetic compatibility
(EMC) – Part 3-3:
Limits – Limitation of voltage changes, voltage fluctuations and
flicker in public
low voltage supply systems, for equipment with
EN 16297-3
rated current
<= 16 A per phase and not subject to conditional connection
EN
16297-3:2012, Pumps – Rotodynamic pumps –Glandless
circulators – Part 3: Energy
efficiency index (EEI) for circulators integrated in products
EN 61000-6-2
EN ISO 14001
61000-6-2:2008/2019, Electromagnetic compatibility (EMC) –
Part 6-2: Generic
standards –Immunity for industrial environments
EN ISO
14001:2015-09, Environmental management systems -
Requirements with guidance
for use
EN 16297-1
EN ISO 14025
16297-1:2012-10, Pumps – Rotodynamic pumps –Glandless
circulators – Part 1:
General requirements and procedures for testing and
calculation of energy DIN EN /ISO
efficiency index (EEI) 14025:2011-10, Environmental labels and declarations — Type
III environmental
declarations — Principles and procedures
EN 15804
EN
15804:2012-04+A1 2013, Sustainability of construction works
— Environmental
Product Declarations — Core rules for the product category of
construction
products
EN 16297-2
16 Environmental Product Declaration - Grundfos Holding A/S - MAGNA3 65-80/100/120 (Cast Iron)
CPR
REGULATION (EU)
No 305/2011 OF THE EUROPEAN PARLIAMENT AND OF
PCR Part A THE COUNCIL of 9 March 2011
laying down harmonised conditions for the marketing of
construction products
and repealing Council Directive 89/106/EEC
Institut Bauen
und Umwelt e.V., Berlin (pub.): Product Category Rules for
Building-Related
Products and Services, Product Category Rules for
Construction Products from
the range of Environmental Product Declarations of Institut
Bauen und Umwelt
(IBU), Part A: Calculation Rules for the Life Cycle Assessment CML 2001
and Requirements
on the Project Report, Version 1.7 (2021)
Impact
assessment characterization factors Institute of Environmental
Sciences, Leiden
University, Netherlands
PCR
Part B
Institut Bauen ECHA candidate
und Umwelt e.V., Berlin (pub.): Product Category Rules for list
Building-Related
Products and Services, Product Category Rules for
Construction Products from
the range of Environmental Product Declarations of Institut Candidate List
Bauen und Umwelt of substances of very high concern (SVHCs) for authorisation,
(IBU), Part B: Requirements on the EPD for Pumps for liquids European
and liquids with Chemicals Agency (ECHA), Helsinki, Finland
solids, Version 1.0 (2018)
Ecoinvent
Ecoinvent v3.5
GaBi ts
Further
references
GaBi ts 9.2.1.68
(database schema 8007)
17 Environmental Product Declaration - Grundfos Holding A/S - MAGNA3 65-80/100/120 (Cast Iron)
SVR
REACH
Advisory Board
(formerly SVA)
Regulation (EC)
No 1907/2006 of the European Parliament and of the Council of
18 December 2006
concerning the Registration, Evaluation, Authorisation and Decision no.
Restriction of 20170712-n
Chemicals (REACH) (Status: 27.06.2018)
The literature referred to in the Environmental Product
Declaration must be listed in full.Standards already fully quoted
in the EPD do not need to be listed here again.
The current version of PCR Part A and PCR Part B of the PCR
document on which they are based must be referenced.
18 Environmental Product Declaration - Grundfos Holding A/S - MAGNA3 65-80/100/120 (Cast Iron)
Publisher
Institut Bauen und Umwelt e.V. +49 (0)30 3087748- 0
Hegelplatz 1 info@ibu-epd.com
10117 Berlin www.ibu-epd.com
Germany
Programme holder
Institut Bauen und Umwelt e.V. +49 (0)30 3087748- 0
Hegelplatz 1 info@ibu-epd.com
10117 Berlin www.ibu-epd.com
Germany
Author of the Life Cycle Assessment
Grundfos Holding A/S +45 87501400
Poul Due Jensens Vej 7 atomic@grundfos.com
8850 Bjerringbro www.grundfos.com
Denmark
Owner of the Declaration
Grundfos Holding A/S +45 87501400
Poul Due Jensens Vej 7 atomic@grundfos.com
8850 Bjerringbro www.grundfos.com
Denmark
19 Environmental Product Declaration - Grundfos Holding A/S - MAGNA3 65-80/100/120 (Cast Iron)
