ENVIRONMENTAL PRODUCT DECLARATION
as per ISO 14025 and EN 15804+A2
Owner of the Declaration IVPU - Industrieverband Polyurethan-Hartschaum e.V.
Publisher Institut Bauen und Umwelt e.V. (IBU)
Programme holder Institut Bauen und Umwelt e.V. (IBU)
Declaration number EPD-IVP-20240423-IBE1-EN
Issue date 29.11.2024
Valid to 28.11.2029
PU thermal insulation boards with mineral fleece facing
IVPU e.V.
www.ibu-epd.com | https://epd-online.com
1. General Information
IVPU e.V. PU thermal insulation boards with mineral fleece
facing
Programme holder Owner of the declaration
IBU – Institut Bauen und Umwelt e.V. IVPU ­ Industrieverband Polyurethan­Hartschaum e.V.
Hegelplatz 1 Heilbronner Str. 154
10117 Berlin 70191 Stuttgart
Germany Germany
Declaration number Declared product / declared unit
EPD­IVP­20240423­IBE1­EN 1 m² of installed PU thermal insulation board with mineral fleece facing (on
both sides), a thickness of 12 cm, a nominal thermal conductivity of 0,025 ­
0,028 W/(m.K) and a delcared value of thermal resistance of Rd = 4,29 –
4,80 (m²•K)/W
This declaration is based on the product category rules: Scope:
Insulating materials made of foam plastics, 01.08.2021 This EPD applies to all declared products of the IVPU's member
(PCR checked and approved by the SVR) companies Karl Bachl GmbH & Co KG, Paul Bauder GmbH & Co KG, IKO
Insulation BV, Kingspan Insulation GmbH & Co KG, Linzmeier
Bauelemente GmbH, puren gmbh, Recticel NV/SA, Steinbacher
Issue date Dämmstoff GmbH, Unilin Insulation bv. The IVPU represents more than
90% of the companies within the German polyurethane insulation products
29.11.2024
market. This EPD is based on weighted averages which have been
determined on the basis of the single values originating from the factories
of the aforementioned manufacturing companies (see section 3.1).
Valid to
The owner of the declaration shall be liable for the underlying information
28.11.2029 and evidence; the IBU shall not be liable with respect to manufacturer
information, life cycle assessment data and evidences.
The EPD was created according to the specifications of EN 15804+A2. In
the following, the standard will be simplified as EN 15804.
Verification
The standard EN 15804 serves as the core PCR
Independent verification of the declaration and data according to ISO
14025:2011
internally X externally
Dipl.­Ing. Hans Peters
(Chairman of Institut Bauen und Umwelt e.V.)
Florian Pronold Prof. Dr. Birgit Grahl,
(Managing Director Institut Bauen und Umwelt e.V.) (Independent verifier)
1 Environmental Product Declaration ­ IVPU e.V. ­ PU thermal insulation boards with mineral fleece facing
2. Product
Name Value Unit
2.1 Product description/Product definition
Gross density 31 ­ 32 kg/m3
Factory made rigid polyurethane foam (PU) products are used
for the thermal insulation of buildings. PU includes both PIR Compressive strength acc. to EN 100 – 150 kPa
and PUR products. The products are manufactured in the form 826
of boards without or with flexible facings. This Product Tensile strength to DIN EN 1607 ≥ 40 kPa
Declaration covers PU insulation boards with mineral fleece Calculation value for thermal
0.026 ­ 0.029 W/(mK)
facings on both sides. conductivity
For the placing on the market of the product in the European
Water vapour diffusion resistance
Union/European Free Trade Association (EU/EFTA) (with the 40 ­ 200 ­
factor acc. to EN 12088
exception of Switzerland) Regulation (EU) No.
Dimensional stability under defined
305/2011 (CPR) applies. The product DS(70/90)3 and
temperature and humidity Class
needs a declaration of performance taking into consideration DS(­20,­)1
conditions DS(TH)i
EN 13165:2016­09 Thermal insulation products for buildings ­
Limiting dimensions of thickness Ti T2 Class
Factory made rigid polyurethane foam (PU) products ­
Specification and the CE­ marking. Thermal conductivity acc. to DIN
0.025 ­ 0.028 W/(mK)
For the design und execution of buidlings the respective EN 13165
Member State's legislation applies. In Germany, the relevant Creep behaviour or permanent
requirements for insulation products are included in DIN 4108­ compressive strength acc. to DIN ≥ 0.02 N/mm2
10. The design value of thermal conductivity is specified in DIN EN 1606
4108­4. Declared value of thermal
4.29 – 4.80 (m²•K)/W
resistance RD
2.2 Application
Thickness at RD = 1 (m²•K)/W 25 – 28 mm
The scope of application of PU rigid foam insulation materials
includes thermal insulation in building construction (e.g. pitched Performance data of the production in accordance with the
roofs, flat roofs, floors, ceilings and exterior walls (inside and declaration of performance with respect to its essential
outside)). characteristics according to DIN 4108-10: 2021-11 (Table 6).
2.3 Technical Data 2.4 Delivery status
For determining technical data, testing methods as stated in EN Polyurethane insulation boards with mineral fleece facings are
13165 are used. The gross density of PU insulation boards with manufactured with plane­parallel surfaces or as tapered
mineral fleece facings for building construction is approx. 31 ­ insulation boards in a thickness range of 20 to 300 mm. This
32 kg/m³. Product Declaration refers to a board thickness of 120 mm. The
format of the boards depends on the planned application. The
Depending on their thickness, the boards obtain nominal width can be up to 1,250 mm and the length up to 12 m. This
thermal conductivity from 0.025 W/(m.K) to 0.028 W/(m.K). product declaration refers to a surface area of 1 m2.
These levels are equivalent to thermal conductivity design
values from 0.026 W/(m.K) up to 0.029 W/(m.K). In addition, the 2.5 Base materials/Ancillary materials
nominal value of the thermal resistance from R = 4.29 The 12 cm PU board with mineral fleece facings consists of
D
(m².K)/W to 4.80 (m².K)/W and the thickness from 25 mm to 28 3.73 kg/m² PU rigid foam and 0.68 kg/m² mineral fleece facings.
Polyurethane rigid foam is formed by the chemical reaction of
mm of the insulation board at R = 1 (m².K)/W can be specified.
D MDI (approx. 58 – 65 %) and polyol (approx. 26 – 31 %),
adding low boiling point blowing agents (approx. 3 – 6 %).
Nominal compressive stress at 10% deformation or
Insulation boards with flexible facings are foamed exclusively
compressive strength is 100 kPa (dh) or 150 kPa (ds) acc. to
with the hydrocarbon pentane. Due to the closed­cell structure,
DIN 4108-10. Higher compressive strength is possible. Nominal
the blowing agent remains within the foam cells. Water (approx.
tensile strength perpendicular to the insulation board plane is
0.2 – 1.5 %), foam stabilisers and catalysts (approx. 2 – 6 %),
40 kPa. Higher tensile strength is possible. The water vapour
as well as flame retardants (Phosphoric acid ester; approx. 2 –
diffusion resistance factor µ of polyurethane rigid foam is
5 %) are added as ancillary materials.
between 40 and 200 acc. to DIN 4108-4. Maximum moisture
absorption of polyurethane rigid foam at diffusion and
The raw materials used for the production of polyurethane rigid
condensation is at approx. 6 % by volume. Water absorption at
foam are mainly obtained from crude oil, undergoing several
total immersion of a 60 mm thick PU insulation board with
production stages. Alternatively, polyols and MDI can be
mineral fleece facings was measured at 1.3 % by volume after
produced, in part, from renewable, plant­based raw materials or
28 days. Moisture absorption after freezing and thawing was
recycled materials. This is not part of this product declaration.
between 2 % and 7 % by volume (measured at insulating
material without facings). Polyurethane rigid foam is a
Polyurethane rigid foam does not contain volatile isocyanates.
distinctive thermosetting material and therefore cannot be
melted.
Under the current Regulation on the Registration, Evaluation,
Constructional data Authorisation and Restriction of Chemicals (REACH)
polyurethane rigid foam is declared as follows:
• Polyurethane rigid foam contains substances listed in
the Candidate List for authorization on 23 January 2024
exceeding 0.1 percentage by mass: no.
• Polyurethane rigid foam contains other carcinogenic,
mutagenic, reprotoxic (CMR) substances in categories
1A or 1B which are not on the candidate list, exceeding
2 Environmental Product Declaration ­ IVPU e.V. ­ PU thermal insulation boards with mineral fleece facing
0.1 percentage by mass: no
• Biocide products were added to this construction 2.11 Environment and health during use
product or it has been The requirements of the Committee for Health­related
treated with biocide products (this then concerns a Evaluation of Building Products (AgBB) are met. Measurements
treated product as defined of emissions using testing chambers in accordance with the
by the (EU) Ordinance on Biocide Products No. relevant testing norms (DIN EN 16516) showed that volatile
528/2012): no organic substances (VVOC, VOC) are only emitted in small
Mineral fleece facings mainly consist of calcium carbonate, quantities.
glass fibres, as well as styrene butadiene rubber (SBR). Regarding the current REACH candidate list, the foam
formulations contain no SVHC substances (see section 2.5).
2.6 Manufacture Polyurethane insulating materials are odourless.
Polyurethane rigid foam insulation boards with flexible mineral
fleece facings are produced in a continuous process on a 2.12 Reference service life
double belt line. In this process, the polyurethane reaction When used properly, the service life time of polyurethane rigid
mixture pours from a mixing head onto the bottom mineral foam corresponds to the service life time of the insulated
fleece facing, where it foams up and glues – still within the construction component or building. The performance of the
line's pressure area – with the top mineral fleece facing. insulation boards stays constant throughout the entire service
After passing the double belt line, the foam boards are cut to life time. Description of the influences on the ageing of the
the desired dimensions. product when applied in accordance with the rules of
technology.
Quality assurance Description of the influences on the ageing of the product when
The declared products are subject to quality controls. Quality applied in accordance with the rules of technology.
assurance is based on surveillance and certification by
independent Notified Bodies.
2.13 Extraordinary effects
2.7 Environment and health during manufacturing Fire
No health protection measures extending beyond the legally­ According to national approvals, polyurethane insulating
mandated work protection measures for industrial businesses materials are classified either as class E or class C acc. to EN
are required during the entire manufacturing process. No 13501-1. Pitched roof constructions with polyurethane
special environmental protection measures apart from the legal insulation over rafters that comply with the classification report
provisions are required. of IBS 316052507-A are classified as REI 30 (fire­retardant).
Roof structures with top­side polyurethane insulation acc. to
2.8 Product processing/Installation DIN 18234-2 meet the fire­protection requirements stated in the
Polyurethane insulation boards can be cut, sawed, milled, and Industrial Building Guideline even for fire containment or fire
abraded with conventional construction tools and portable fighting sections with a roof surface of more than 2,500 m².
machines. In general, the boards are fixed mechanically
(pitched and flat roofs, cavity core insulation). Alternatively, PU In case of fire, PU rigid foam does not tend to smoulder. When
insulation boards can be laid loosely, e.g. on floors. Observing exposed to heat, PU rigid foam carbonizes without dripping off
the manufacturer's recommendations, it is also possible to glue burning droplets. When burning, sooty products, water vapour,
the boards together by using either hot­setting or cold­setting carbon monoxide, carbon dioxide, nitrogen oxides, as well as
adhesives. Joints between cut insulation boards on roof ridges, hydrogen cyanide are formed as it is the case e. g. for sheep
hips or valleys are to be sealed with polyurethane in­situ foam wool. The toxicity of the combustion gases mainly depends on
without thermal bridges. While sawing, abrading, and milling the amount of burned material in relation to the size of the room
insulation boards, dust is generated. If there is no sufficient in which the gases are distributed. It also depends on the
ventilation, workers who carry out these processes have to ventilation conditions in the affected area.
protect themselves by wearing an appropriate dust filter mask
(see leaflet of the 'Berufsgenossenschaft der Chemischen
Fire Protection
Industrie' on respiratory protection). Dust concentration in the
Name Value
air (general limit of dust concentration as per TRGS 900,
Technische Regeln für Gefahrstoffe) must not exceed the Building material class E ­ C
following values: Burning droplets d0, none
• 10 mg/m³ (measured as inhalable fraction) Smoke gas development s1 ­ s3
• 1.25 mg/m³ (measured as alveolar fraction)
These limits are time­weighted averages assumingan 8­hour Water
exposure per day, 5 days a week, during working lifetime. Due to the predominant closed­cell structure, insulating
Cutting leftovers can be treated in a municipal waste materials made of polyurethane rigid foam absorb water only in
incernation plant with energy recovery or they can be subject to small quantities. They are not hygroscopic, i.e. they do not
a separate collection and a mechanical recycling process. absorb water vapour from the air. When unexpectedly exposed
to water (e.g. flood), only very small amounts of soluble
2.9 Packaging
substances are emitted.
Mainly, plastic foils and EPS or PU wedges are used as
packaging material. The plastic foils can be recycled whereas
Mechanical destruction
the PU wedges can be reused in the form of PU press plates.
The disintegration of the poduct by mechanical processes does
not have relevant effects on the environment.
2.10 Condition of use
Under normal conditions of use, the material does not undergo 2.14 Re-use phase
any changes in terms of substance during its service life time.
Dismantling polyurethane insulating materials as well as sorting
Polyurethane is resistant to most chemicals used in
and waste identifying can be done without difficulties, since
construction and does not rot.
they are usually mounted mechanically or laid loosely. Clean
and undamaged polyurethane insulation boards can be reused
3 Environmental Product Declaration ­ IVPU e.V. ­ PU thermal insulation boards with mineral fleece facing
as well as recycled mechanically or chemically (glycolysis). frames or thermal bridges.
Glycolysis means that polyurethane rigid foam waste is
transformed into a fluid substance called glycolysis polyol, 2.15 Disposal
which can be used again as raw material in the production of According to the Waste Catalogue Ordinance, polyurethane
polyurethane. insulating material shall not be disposed of without prior
When reutilised from mechanical material recycling, treatment. The waste code for construction waste is 170604.
polyurethane rigid foam waste is used to produce press boards. During thermal treatment, the energy content of the insulation
In this process, cutting and mounting leftovers, as well as material can be recovered.
construction waste, are mechanically shredded and
2.16 Further information
subsequently pressed into board­shaped products while adding
binding agents. PU pressed adhesive boards are a high­quality Please visit www.ivpu.de and www.daemmt­besser.de for
material that are used, among others, to insulate window further information on PU insulating materials.
3. LCA: Calculation rules
been considered in this EPD.
3.1 Declared Unit
The declared unit is 1 m² of installed PU thermal insulation 3.4 Cut-off criteria
board with mineral fleece facing (on both sides) and has the In this study, all available data from the production are taken
following specifications: into account, i.e. all used raw
materials, used thermal energy, as well as electrical power
Declared unit
consumption.
Name Value Unit
Therefore, even materials and power consumption levels that
Declared unit 1 m2 have a share of less than 1 % are considered.
Gross density of the PU foam 31.12 kg/m3 It can be assumed that all neglected processes put together
account for no more than 5 % of total power and mass
Grammage 4.42 kg/m2
consumption.
Layer thickness 0.12 m
The manufacturers have provided data on transport
Design value of thermal conductivity 0.026 W/(m•K) expenditures for all relevant material flows. Machinery and
Thermal resistance (R­value) 4.29­4.80 m²•W/K installations required for production are neglected.
Other declared units are allowed if the conversion is shown 3.5 Background data
transparently.
Background data originates from the Sphera LCA FE (GaBi ts)
software database CUP 2023.2 from Sphera. The power mix
This EPD is based on weighted averages, which have been
with different countries has been used. The last revision of the
determined on the basis of the single values originating from
used data was less than 6 years ago.
the factories of the 9 IVPU members. Average energy
consumption for producing PU boards has been weighted 3.6 Data quality
according to the quantities of produced PU rigid foam in m3. The data used are primary data originating from the industry
Raw material consumption has been weighted according to and were gathered by the IVPU in 2018. 9 IVPU members (see
used quantities in kg. Rigid foam waste is weighted according above) participated in this data gathering. The IVPU represents
to the quantities of produced PU rigid foam in m3, whereas more than 90% of the companies within the German
facing waste is weighted according to used quantities of facings polyurethane insulating materials market. This EPD is based on
in m2. weighted averages, which have been determined on the basis
of the single values originating from the factories of the
3.2 System boundary
aforementioned manufacturing companies.
The type of EPD according to EN15804 is cradle to gate with The data's quality as well as its temporal, technological and
options, modules C1–C4, and module D. geographical representativeness significance can be classified
The life cycle assessment considers the following steps of the as good.
life cycle:
3.7 Period under review
• Production and supply of raw materials (A1)
The data basis is based on production data from 2018.
• Transporting raw materials (A2)
The used quantities of raw materials, energy, as well as
• Production including packaging (A3)
ancillary materials and fuels are averages compiled over a time
• Transport to construction site (A4)
span of 12 months.
• Installation in buildings (thermal treatment of packaging
waste) (A5)
3.8 Geographic Representativeness
• Transport to End­of­Life (C2)
Land or region, in which the declared product system is
• Waste treatment: energy for shredders (C3)
manufactured, used or handled at the end of the product´s
• Thermal treatment (PU foam) (C3)
lifespan: Germany
• Recycling or use potentials beyond the system's
boundary (D).
3.9 Allocation
3.3 Estimates and assumptions
When thermally treated in waste incineration plants (MVA),
For all inputs, specific Sphera LCA FE (GaBi ts) data sets were
recycling as well as use potentials beyond the system boundary
available.
for power and thermal energy of module A5 and C3 are taken
Currently, waste from PU foam production generated in
into account in module D in an input­specific manner
construction sites are handled using mainly material recycling
considering elemental composition as well as calorific values.
(see 2.15).
Due to manufacturing locations and distribution throughout all
Using a worst­case approach, only the incineration and the
of Europe, the substitution processes refer to reference area
consequent energy benefit beyond the system boundary have
EU­27.
4 Environmental Product Declaration ­ IVPU e.V. ­ PU thermal insulation boards with mineral fleece facing
the product­specific characteristics of performance, are taken
3.10 Comparability into account. The used background database is Sphera LCA
Basically, a comparison or an evaluation of EPD data is only FE (GaBi ts), CUP 2023.2.
possible if all the data sets to be compared were created
according to EN 15804 and the building context, respectively
4. LCA: Scenarios and additional technical information
Installation in buildings (A5)
Characteristic product properties of biogenic carbon
The biogenic carbon content declared is provided below. No Name Value Unit
biogenic carbon content exists in the product, only packaging Packaging waste 0.63 kg
materials.
Information on describing the biogenic carbon content at
End of life cycle (C1-C4)
factory gate
Name Value Unit
Name Value Unit
Waste processing (C3) energy for shredders 0.883 MJ
kg
Biogenic carbon content in product ­ Reuse ­ kg
C
Recycling 0.68 kg
Biogenic carbon content in accompanying kg
packaging 0.0376 C Energy recovery 3.74 kg
Landfilling ­ kg
Note: 1 kg of biogenic carbon is equivalent to 44/12 kg of CO2.
Module C1 considers a manual demolition (without any
burden). Upon removal from the building, products are
The following technical scenario information is used to calculate assumed to be transported 100 km (module C2) to a recycling
the declared modules. The values refer to the declared unit of 1 facility. The foam waste in the EoL phase is sent to a waste
m² of installed PU thermal insulation board with mineral fleece incineration plant.
facing.
The waste is shredded and incinerated. These processes are
grouped to module C3. Resulting potential benefits for
Transport to construction site (A4)
electricity and thermal energy due to the incineration are
Name Value Unit
grouped to module D.
Litres of fuel 0.0288 l/100km
Transport distance 500 km Aluminum facings are recycled. The recycling including the
Gross density of products transported 31.12 kg/m3 recycling effort and the potential benefits are addressed in
module D.
Capacity utilisation (including empty runs) 85 %
5 Environmental Product Declaration ­ IVPU e.V. ­ PU thermal insulation boards with mineral fleece facing
5. LCA: Results
DESCRIPTION OF THE SYSTEM BOUNDARY (X = INCLUDED IN LCA; MND = MODULE OR INDICATOR NOT DECLARED; MNR
= MODULE NOT RELEVANT)
Benefits and
Construction loads beyond
Product stage Use stage End of life stage
process stage the system
boundaries
la ire ta m w a Ry lp p u s tro p s n a rT g n iru tc a fu n a M e h t m o rf tro p s n a rTe tis e h t o t e ta g y lb m e s s A e s U e c n a n e tn ia M ria p e R tn e m e c a lp e R tn e m h s ib ru fe R y g re n e la n o ita re p Oe s u re ta w la n o ita re p Oe s u n o itc u rts n o c ­e Dn o itilo m e d tro p s n a rT g n is s e c o rp e ts a W la s o p s iD ­e s u e R­y re v o c e R­g n ilc y c e Rla itn e to p
A1 A2 A3 A4 A5 B1 B2 B3 B4 B5 B6 B7 C1 C2 C3 C4 D
X X X X X MND MND MNR MNR MNR MND MND X X X X X
RESULTS OF THE LCA - ENVIRONMENTAL IMPACT according to EN 15804+A2: 1 m² of installed PU insulation board with
mineral fleece facing
Parameter Unit A1-A3 A4 A5 C1 C2 C3 C4 D
GWP­total kg CO 2 eq 1.2E+01 4.85E­01 2.03E­01 0 9.54E­02 8.52E+00 9.04E­03 ­3.17E+00
GWP­fossil kg CO 2 eq 1.21E+01 4.8E­01 2.01E­01 0 9.43E­02 8.52E+00 9.01E­03 ­3.16E+00
GWP­biogenic kg CO 2 eq ­3.73E­02 1.12E­03 2.19E­03 0 2.2E­04 1.17E­03 2.71E­07 ­1.45E­02
GWP­luluc kg CO 2 eq 1.05E­02 4.53E­03 2.09E­07 0 8.92E­04 2.21E­05 2.84E­05 ­2.06E­04
ODP kg CFC11 eq 1.45E­11 4.29E­14 9.8E­15 0 8.43E­15 2.14E­12 2.32E­14 ­2.49E­11
AP mol H+ eq 2.35E­02 6.39E­04 2.29E­05 0 1.26E­04 5.07E­03 6.48E­05 ­3.95E­03
EP­freshwater kg P eq 4.75E­05 1.79E­06 2.36E­09 0 3.51E­07 4.8E­07 1.84E­08 ­5.13E­06
EP­marine kg N eq 6.38E­03 2.25E­04 5.98E­06 0 4.42E­05 2.41E­03 1.67E­05 ­1.16E­03
EP­terrestrial mol N eq 6.59E­02 2.7E­03 1.11E­04 0 5.31E­04 2.77E­02 1.84E­04 ­1.24E­02
kg NMVOC
POCP 3.48E­02 5.51E­04 1.69E­05 0 1.08E­04 6.19E­03 5.05E­05 ­3.22E­03
eq
ADPE kg Sb eq 1.3E­06 3.18E­08 9.13E­11 0 6.25E­09 1.87E­08 4.23E­10 ­2.27E­07
ADPF MJ 3.14E+02 6.66E+00 2.5E­02 0 1.31E+00 3.88E+00 1.22E­01 ­5.83E+01
m3 world eq
WDP 1.78E+00 5.64E­03 1.83E­02 0 1.11E­03 8.48E­01 1E­03 ­3.01E­01
deprived
GWP = Global warming potential; ODP = Depletion potential of the stratospheric ozone layer; AP = Acidification potential of land and water; EP =
Eutrophication potential; POCP = Formation potential of tropospheric ozone photochemical oxidants; ADPE = Abiotic depletion potential for non­fossil
resources; ADPF = Abiotic depletion potential for fossil resources; WDP = Water (user) deprivation potential)
RESULTS OF THE LCA - INDICATORS TO DESCRIBE RESOURCE USE according to EN 15804+A2: 1 m² of installed PU
insulation board with mineral fleece facing
Parameter Unit A1-A3 A4 A5 C1 C2 C3 C4 D
PERE MJ 1.59E+01 4.71E­01 1.36E+00 0 9.26E­02 1.41E+00 1.98E­02 ­1.7E+01
PERM MJ 1.35E+00 0 ­1.35E+00 0 0 0 0 0
PERT MJ 1.73E+01 4.71E­01 6.26E­03 0 9.26E­02 1.41E+00 1.98E­02 ­1.7E+01
PENRE MJ 1.96E+02 6.67E+00 2.33E+01 0 1.31E+00 9.91E+01 1.22E­01 ­5.83E+01
PENRM MJ 1.18E+02 0 ­2.33E+01 0 0 ­9.52E+01 0 0
PENRT MJ 3.15E+02 6.67E+00 2.51E­02 0 1.31E+00 3.88E+00 1.22E­01 ­5.83E+01
SM kg 0 0 0 0 0 0 0 0
RSF MJ 0 0 0 0 0 0 0 0
NRSF MJ 0 0 0 0 0 0 0 0
FW m3 7.71E­02 5.19E­04 4.28E­04 0 1.02E­04 2.03E­02 3.07E­05 ­1.38E­02
PERE = Use of renewable primary energy excluding renewable primary energy resources used as raw materials; PERM = Use of renewable primary
energy resources used as raw materials; PERT = Total use of renewable primary energy resources; PENRE = Use of non­renewable primary energy
excluding non­renewable primary energy resources used as raw materials; PENRM = Use of non­renewable primary energy resources used as raw
materials; PENRT = Total use of non­renewable primary energy resources; SM = Use of secondary material; RSF = Use of renewable secondary fuels;
NRSF = Use of non­renewable secondary fuels; FW = Use of net fresh water
RESULTS OF THE LCA – WASTE CATEGORIES AND OUTPUT FLOWS according to EN 15804+A2:
1 m² of installed PU insulation board with mineral fleece facing
Parameter Unit A1-A3 A4 A5 C1 C2 C3 C4 D
HWD kg 9.84E­08 2.47E­11 6.82E­13 0 4.86E­12 6.3E­11 2.65E­12 ­3.15E­09
NHWD kg 2.61E­01 9.62E­04 8.42E­04 0 1.89E­04 4.36E­02 6.09E­01 ­2.88E­02
RWD kg 4.36E­03 8.63E­06 1.47E­06 0 1.7E­06 3.55E­04 1.39E­06 ­4.51E­03
CRU kg 0 0 0 0 0 0 0 0
MFR kg 0 0 0 0 0 0 0 0
MER kg 0 0 0 0 0 0 0 0
EEE MJ 0 0 4.13E­01 0 0 1.46E+01 0 0
6 Environmental Product Declaration ­ IVPU e.V. ­ PU thermal insulation boards with mineral fleece facing
EET MJ 0 0 7.34E­01 0 0 2.62E+01 0 0
HWD = Hazardous waste disposed; NHWD = Non­hazardous waste disposed; RWD = Radioactive waste disposed; CRU = Components for re­use;
MFR = Materials for recycling; MER = Materials for energy recovery; EEE = Exported electrical energy; EET = Exported thermal energy
RESULTS OF THE LCA – additional impact categories according to EN 15804+A2-optional:
1 m² of installed PU insulation board with mineral fleece facing
Parameter Unit A1-A3 A4 A5 C1 C2 C3 C4 D
Disease
PM 2.01E­07 5.3E­09 1.22E­10 0 1.04E­09 1.51E­08 7.97E­10 ­3.35E­08
incidence
IR kBq U235 eq 4.35E­01 1.25E­03 2.37E­04 0 2.45E­04 5.83E­02 1.6E­04 ­7.5E­01
ETP­fw CTUe 1.08E+02 4.69E+00 9.66E­03 0 9.22E­01 1.11E+00 6.58E­02 ­8.14E+00
HTP­c CTUh 4E­09 9.45E­11 1.28E­12 0 1.86E­11 8.24E­11 1.02E­11 ­6.46E­10
HTP­nc CTUh 1.44E­07 4.17E­09 1.07E­11 0 8.21E­10 1.25E­09 1.08E­09 ­1.59E­08
SQP SQP 4.58E+01 2.78E+00 7.71E­03 0 5.46E­01 1.14E+00 2.96E­02 ­1.12E+01
PM = Potential incidence of disease due to PM emissions; IR = Potential Human exposure efficiency relative to U235; ETP­fw = Potential comparative
Toxic Unit for ecosystems; HTP­c = Potential comparative Toxic Unit for humans (cancerogenic); HTP­nc = Potential comparative Toxic Unit for humans
(not cancerogenic); SQP = Potential soil quality index
Disclaimer 1 – for the indicator “Potential Human exposure efficiency relative to U235”. This impact category deals mainly with the
eventual impact of low­dose ionizing radiation on human health of the nuclear fuel cycle. It does not consider effects due to possible
nuclear accidents, occupational exposure or radioactive waste disposal in underground facilities. Potential ionizing radiation from the
soil, radon and from some construction materials is also not measured by this indicator.
Disclaimer 2 – for the indicators “abiotic depletion potential for non­fossil resources”, “abiotic depletion potential for fossil resources”,
“water (user) deprivation potential, deprivation­weighted water consumption”, “potential comparative toxic unit for ecosystems”,
“potential comparative toxic unit for humans – cancerogenic”, “Potential comparative toxic unit for humans ­ not cancerogenic”,
“potential soil quality index”. The results of this environmental impact indicator shall be used with care as the uncertainties on these
results are high as there is limited experience with the indicator.
6. LCA: Interpretation
Modules A1­A3: The environmental impacts during the originates from using primary energy generated from MVAs,
production stage are mainly determined by raw material which burn PU cores in order to generate power and steam.
production and processing in Module A1. For nearly all
categories, these impacts can mostly be attributed to the PU The LCA results show high robustness since the primary data,
foam (80 % ­ 90 %) and to a lesser extent to the mineral fleece they are based on, do not show any outliers in terms of energy
facings (<10 %). More specifically, the results are mainly driven consumption and product's composition while comparing the
the production of MDI and polyols in almost all indicators except contributing companies and sites. All background data are
for ODP and POCP, where the impacts can mainly be attributed sourced from Sphera LCA FE (GaBi ts) databases. With the
to the power mix and the other production expenses, used data sets a good overall representativity with regards to
respectively. completeness, geographical coverage and technological
coverage is ensured.
Module D: The utilization potential for the next product system
7. Requisite evidence
7.1 VOC emissions
Emission tests on PU boards with mineral fleece facings found 7.2 Isocyanate emission
that the VOC values are significantly below the limits In the analysis conducted by the Fraunhofer Institut für
determined by the AgBB scheme (PU Europe Technical Holzforschung, Wilhelm­Klauditz­Institut WKI (Test report No.
Dossier). The tests were conducted by the research 861-98), no isocyanate emission could be detected in the 1m³
organisations Eurofins (Denmark), VTT (Finland) and test chamber. SUPELCO cartridges have been used for
Fraunhofer WKI (Germany), Test report No. MAIC-2016-3308, detecting MDI. The detection limit is at 10 ng/m³.
among others.
7.3 Formaldehyde
VOC emissions
Emission tests on PU insulation boards only detected very
Name Value Unit
small quantities of formaldehydes (< 3 μg/m³ (PU Europe
TVOC (C6 ­ C16) 0 ­ 100 μg/m3 Technical Dossier)). This is significantly below the threshold
Sum SVOC (C16 ­ C22) 0 ­ 10 μg/m3 value of 120 μg/m³ (Class E1).
R (dimensionless) 0 ­ 0.5 ­
VOC without NIK 0 ­ 100 μg/m3
Carcinogenic Substances ­ μg/m3
8. References
Standards in buildings ­ Part 4: Hygrothermal design values.
DIN 4108-4 DIN 4108-10
DIN 4108­4:2020­­11, Thermal insulation and energy economy DIN 4108­10:2021­­11, Thermal insulation and energy economy
7 Environmental Product Declaration ­ IVPU e.V. ­ PU thermal insulation boards with mineral fleece facing
in buildings ­ Part 10: Application­related requirements for Declarations (EPD) ­ Product Category Rules (PCR)
thermal insulation materials ­ Factory­made products. complementary to EN 15804 for factory made and in­situ
formed products
EN 12091
EN 12091:2013­­06, Thermal insulating products for building EN ISO 14025
applications ­ Determination of freeze­thaw resistance. EN ISO 14025:2011, Environmental labels and declarations —
Type III environmental declarations —
EN 13165 Principlesandprocedures.
EN 13165:2016­­09, Thermal insulation products for buildings –
Factory­made rigid polyurethane foam (PU) products ­ Further References
Specification; German version EN 13165:2012. (This norm
covers polyurethane rigid foam (PUR) and polyisocyanurate AgBB
rigid foam (PIR)). Evaluation scheme for VOCs from construction products;
approach for assessing health risks caused by volatile organic
DIN EN 13501-1 compounds (VOCs and SVOCs) from construction products,
EN 13501­1:2019­­05, Fire classification of construction version 2021.
products and building elements ­ Part 1: Classification using
data from reaction to fire tests; German version EN 13501­ Waste Catalogue Ordinance
1:2007+A1:2010.
Waste Catalogue Ordinance of 10 Dec 2001 (Federal Law
EN 14308 Gazette I p. 3379), last amended by Article 2 of the Ordinance
EN 14308:2016­­03, Thermal insulation products for building of 24 July 2002 (Federal Law Gazette 2833):
equipment and industrial installations ­ Factory made rigid CPR
polyurethane foam (PUR) and polyisocyanurate foam (PIR) Regulation (EU) No. 305/2011 of the European Parliament and
products. of the Council of 9 March 2011 laying down harmonised
condition for the marketing of construction products and
EN 15801 repealing Council Directive 89/106/EC.
EN 15801:2010­­04, Conservation of cultural property ­ Test
methods ­ Determination of water absorption by capillarity. EXCLI Journal
Hoffmann, Hans­Dieter; Schupp, Thomas: 'Evaluation of
EN 1606 consumer risk resulting from exposure against MDI from
EN 1606:2013­­05, Thermal insulating products for building polyurethane foam,' scientific article, published in the EXCLI
applications ­ Determination of compressive creep. Journal in 2009.
EN 1607 IBU 2021
EN 1607:2013­­05, Thermal insulating products for building Institut Bauen und Umwelt e.V.: General Instructions for the
applications ­ Determination of tensile strength perpendicular to EPD programme of Institut Bauen und Umwelt e.V., version 2.0,
faces. Berlin: Institut Bauen und Umwelt e.V., 2021 www.ibu­­epd.com
EN 16516 IBS 316052507-A
EN 16516:2020­­10, Construction products: Assessment of IBS Linz: Test report No. 316052507­A, dated 06.04.2017
release of dangerous substances ­ Determination of emissions (IVPU), "Report on the classification of fire resistance of a rafter
into indoor air. roof with PU over­rafter insulation".
DIN 18234-2 IVPU
DIN 18234­2:2018­­05, Fire safety of large roofs for buildings ­ IVPU news: Article "Report on emission of volatile components
Fire exposure from below ­ Part 2: List of roofs which fulfil the from PUR rigid foam insulating materials," no. 64 dated June
requirements of DIN 18234­1; roof areas without openings. 1999.
EN 29052-1 PCR Part A
EN 29052­1:1992­­08, Acoustics; determination of dynamic PCR ­ Part A: Calculation rules for the Life Cycle Assessment
stiffness; part 1: materials used under floating floors in and Requirements on the Background Report, version 1.3,
dwellings. Institut Bauen und Umwelt e.V., 2021.
EN 826 PCR Part B
EN 826:2013­­05, Thermal insulating products for building PCR ­ Part B: Requirements of the EPD for foam
applications ­ Determination of compression behaviour. plasticsinsulation materials, v8, 2021
www.bau­­umwelt.de
EN 12088
EN 12088:2013, Thermal insulating products for building PU Europe Technical Dossier
applications ­ Determination of long term water absorption by Technical Dossier for amendment to mandate M103
diffusion. VOC/SVOC emissions, doc. 13/241, 2013.
EN 15804 Ordinance on Biocide Products No. 528/2012
EN 15804:2012+A2:2019+AC:2021, Sustainability of Regulation (EU) No. 528/2012 of the European Parliament and
construction works — Environmental Product Declarations Core of the Council of 22 May 2012 concerning the making available
rules for the product category of construction products. on the market and use of biocidal products.
prEN 16783:2022-12 - draft REACH
Thermal insulation products ­ Environmental Product Regulation (EC) No. 1907/2006 of the European Parliament
8 Environmental Product Declaration ­ IVPU e.V. ­ PU thermal insulation boards with mineral fleece facing
and of the Council dated 18th December 2006 on the Europe), "Evaluation of emissions data from PU insulation on a
Registration, Evaluation, Authorisation and Restriction of Commission proposal for the classification of emissions from
Chemicals (REACH). building products in the European Union".
Sphera LCA FE (GaBi ts) Test report No. 861-98
Sphera LCA for Experts, LCA FE, software­ system and Fraunhofer Institut für Holzforschung, Wilhelm­Klauditz­Institut
databases, Managed LCA content MLC (fka GaBi database), (WKI): Test report No. 861­98, dated 07.12.1998 (IVPU), "Test
University of Stuttgart and Sphera Solutions GmbH, 2023 CUP reports on emissions of volatile components from polyurethane
Version: 2023.2, MLC data set documentation under insulating materials".
https://sphera.com/product­sustainability­gabi­data­search/
(March 2024). TRGS 900
Federal Institute for Occupational Safety and Health: Technical
Test report No. MAIC-2016-3308 Rules for Hazardous Substances (TRGS) 900, Threshold
Fraunhofer Institut für Holzforschung, Wilhelm­Klauditz­Institut values for workplaces, 2006, last modified 15.01.2024.
(WKI): Test report No. MAIC­2016­3308, dated 04.08.2016 (PU
9 Environmental Product Declaration ­ IVPU e.V. ­ PU thermal insulation boards with mineral fleece facing
Publisher
Institut Bauen und Umwelt e.V. +49 (0)30 3087748­ 0
Hegelplatz 1 info@ibu­epd.com
10117 Berlin www.ibu­epd.com
Germany
Programme holder
Institut Bauen und Umwelt e.V. +49 (0)30 3087748­ 0
Hegelplatz 1 info@ibu­epd.com
10117 Berlin www.ibu­epd.com
Germany
Author of the Life Cycle Assessment
Sphera Solutions GmbH +49 (0)711 341817­0
Hauptstraße 111­ 113 info@sphera.com
70771 Leinfelden­Echterdingen www.sphera.com
Germany
Owner of the Declaration
IVPU ­ Industrieverband Polyurethan­Hartschaum +49 711 29 17 16
e.V. ivpu@ivpu.de
Heilbronner Str. 154 http://www.ivpu.de/
70191 Stuttgart
Germany
10 Environmental Product Declaration ­ IVPU e.V. ­ PU thermal insulation boards with mineral fleece facing
