ENVIRONMENTAL PRODUCT DECLARATION
as per ISO 14025 and EN 15804+A1
Owner of the Declaration
Programme holder Institut Bauen und Umwelt e.V. (IBU)
Publisher Institut Bauen und Umwelt e.V. (IBU)
Declaration number EPD-ARC-20220173-CBC1-EN
Issue date 25.07.2022
Valid to 24.07.2027
XCarb® Recycled and Renewably Produced Hot Rolled Coils
ArcelorMittal Europe
www.ibu-epd.com | https://epd-online.com
Umwelt Produktdeklaration Name des Herstellers – Name des Produkts
General Information
ArcelorMittal Europe XCarb® Recycled and Renewably
Produced Hot Rolled Coil
Programme holder Owner of the declaration
IBU – Institut Bauen und Umwelt e.V. ArcelorMittal Europe – Flat Products
Hegelplatz 1 24-26 Boulevard d’Avranches
10117 Berlin L-1160 Luxembourg
Germany Luxembourg
Declaration number Declared product / declared unit
EPD-ARC-20220173-CBC1-EN The declared unit is 1 ton of hot rolled steel coil.
This declaration is based on the product Scope:
category rules: This declaration applies to 1 metric tonne of XCarb®
Structural steels, 11.2017 Recycled and Renewably Produced Hot Rolled Coils
(PCR checked and approved by the SVR) produced at ArcelorMittal Sestao.
Issue date The Life Cycle Assessment is based on data collected
25.07.2022 in 2021 for deliveries based on Guarantee of Origins
renewable electricity supply.
Valid to
24.07.2027 The owner of the declaration shall be liable for the
underlying information and evidence; the IBU shall not
be liable with respect to manufacturer information, life
cycle assessment data and evidences.
The EPD was created according to the specifications
of EN 15804+A1. In the following, the standard will be
simplified as EN 15804.
Verification
The standard EN 15804 serves as the core PCR
Independent verification of the declaration and data
according to ISO 14025:2011
Dipl. Ing. Hans Peters internally x externally
(chairman of Institut Bauen und Umwelt e.V.)
Dr. Alexander Röder Matthias Klingler
(Managing Director Institut Bauen und Umwelt e.V.)) (Independent verifier)
Product
Product description/Product definition manufacturers for shaping into finished products.
This Environmental Product Declaration refers to
XCarb® Recycled and Renewably Produced Hot The mean thickness value is at 5 mm but the
Rolled Coils used for any commercial and structural declaration refers to hot rolled steel coils between 985
applications, including Amstrong® high strength steel and 1550 mm wide and 1 to 12.74 mm thick.
range. XCarb® Recycled and Renewably
Produced Hot Rolled Coils refer to Black or Pickled & For the placing on the market of the product in the
Oiled coils. The EPD results reflect the volume- European Union/European Free Trade Association
weighted share of these coils (60 % Black, 40 % (EU/EFTA) (with the exception of Switzerland)
Pickled & Oiled). Regulation (EU) No. 305/2011 (CPR) applies. The
product has a declaration of performance taking into
XCarb® Recycled and Renewably Produced Hot consideration EN 10025-1 - Hot rolled products of
Rolled Coils are produced at ArcelorMittal Sestao in structural steels - Part 1: General technical delivery
Spain; their production is based on Electric Arc conditions. For the application and use, the respective
Furnace and Compact Strip Production processes with national provisions apply.
renewable electricity supply with Guarantee of Origins.
Other European standards concerning Hot Rolled Coils
Products are continuously rolled at high temperatures could also be used by manufacturers for various
going through a series of stands of rotating cylinders. pieces or components:
Steel alloy composition and process parameters are  EN 10149-2 - Hot rolled flat products made of
set to guarantee the required grade. The coils are then high yield strength steels for cold-forming.
delivered, Black or Pickled & Oiled, to processors and
2 Environmental Product Declaration ArcelorMittal – XCarb® Recycled and Renewably Produced Hot Rolled Coils
 General technical delivery conditions can be Constructional data
considered as specified in EN 1993-1-3 - Name Value Unit
Density 7850 kg/m3
Eurocode 3 - Design of steel structures - Part
Modulus of elasticity 210000 N/mm2
1-3: General rules - Supplementary rules for
Thermal conductivity 48 W/(mK)
cold-formed members and sheeting.
Melting point 1650 °C
 Drawing steels according to EN 10111 and
Yield strength (min-max) 170-700 MPa
other special grades according to EN ISO
683.
Performance data of the product are in accordance
with the declaration of performance with respect to its
These products, not covered by EN 10025, are not
essential characteristics according to EN 10025-1 - Hot
under CPR and do not require CE marking to be
rolled products of structural steels - Part 1: General
placed on the market.
technical delivery conditions.
Characteristics are also specified in the American
Base materials/Ancillary materials
standard ASTM G101-04:2015 (American Society for
The basic materials for the manufacture of
Testing and Materials) for hot-rolled material.
ArcelorMittal’s steel coil are non-alloyed and fine grain
steel. Different steel grades and qualities are possible,
Application
according to standards previously mentioned.
XCarb® Recycled and Renewably Produced Hot
Rolled Coils can be used in various applications, such
The base material for XCarb® Recycled and
as:
Renewably Produced Hot Rolled Coils is iron.
 Construction: structural or non-structural
Variations in carbon content and alloying elements
welded sections, façade & cladding, roofing,
modify the chemical and physical properties of steel
sunscreens & shades; such as strength, durability and corrosion resistance.
 Road equipment: safety barriers, protection Such material additions make up a small percentage
equipment, sound insulation wall panels; by mass of the final product.
 Art sculpture & Other industrial applications
This product contains substances listed in the
such as containers, filters, etc.
candidate list (date: 02.06.2022) exceeding 0.1
percentage by mass: no.
They are delivered as wide coils that can be processed
in slit coils or cut-to-length sheets. They can be further Reference service life
processed by all conventional manufacturing A reference service life for XCarb® Recycled and
operations used for hot rolled steel: mechanical and Renewably Produced Hot Rolled Coils is not declared.
thermal cutting, bending, drawing, roll-forming,
stamping, welding, etc. Hot rolled coils are used in construction with many
different application purposes. The lifetime therefore
Technical Data will be limited by the application and corresponding
XCarb® Recycled and Renewably Produced Hot service.
Rolled Coils cover a full range of products in
compliance with the EN 10025, EN 10149, EN 10111 At the end of life, they will be recovered and recycled
and EN ISO 683 to meet various requirements. into a new steel product.
LCA: Calculation rules
Declared Unit Modules A1-A3 of the XCarb® Recycled and
The declaration refers to the functional unit of 1 metric Renewably Produced Hot Rolled coil production
ton XCarb® Recycled and Renewably Produced Hot include:
Rolled steel coil, black or pickled & oiled, packed and  The provision of resources, additives, and
ready to be transported from ArcelorMittal to its energy
clients as specified in Part B requirements on the EPD.
 Transport of resources and additives to the
production site
Declared unit
Name Value Unit  Production processes on site include energy,
Declared unit 1 t production of additives, disposal of production
Density 7850 kg/m3 residues, and consideration of related
emissions.
 Recycling of production/manufacturing scrap.
Steel scrap is assumed to reach the end-of-
System boundary
waste status once it is shredded and sorted,
Type of the EPD: cradle-to-gate - with options.
Module A1-A3, Module C3, Module C4 and Module D thus becoming input to the product system in
were considered. the inventory.
3 Environmental Product Declaration ArcelorMittal – XCarb® Recycled and Renewably Produced Hot Rolled Coils
Module C3 takes into account the sorting and context, respectively the product-specific
shredding of after-use steel, as well as the non- characteristics of performance, are taken into account.
recovered scrap due to sorting efficiency which is
landfilled. A conservative value of 2% landfill is For life cycle modelling of the considered
considered (Module C4). products, GaBi ts software version 10.6.1.35 was used
with GaBi database 2022.2. This database contains
Module D refers to the end-of-life of the XCarb® consistent and documented datasets available in Gabi
Recycled and Renewably Produced Hot Rolled coil, Documentation
including reuse and recycling.
Materials and chemicals used were modelled using the
Comparability allocation rule most suitable for the respective product.
Basically, a comparison or an evaluation of EPD data For further information on a specific product
is only possible if all the data sets to be compared check Gabi Documentation and Worldsteel Association
were created according to EN 15804 and the building Methodology Report.
LCA: Scenarios and additional technical information
Current practice for the average XCarb® Recycled and
Renewably Produced Hot Rolled coil consists of 98 %
recycling and 2 % landfill according to the European
Commission Technical Steel Research.
End of life (C1-C4)
Name Value Unit
Recycling 980 kg
Landfilling 20 kg
Sorting and shredding of after-use steel, as well as
non-recovered scrap.
Reuse, recovery and/or recycling potentials (D),
relevant scenario information
Name Value Unit
Recycling 980 kg
4 Environmental Product Declaration ArcelorMittal – XCarb® Recycled and Renewably Produced Hot Rolled Coils
LCA: Results
DESCRIPTION OF THE SYSTEM BOUNDARY (X = INCLUDED IN LCA; MND = MODULE NOT DECLARED;
MNR = MODULE NOT RELEVANT)
BENEFITS AND
CONSTRUCTI LOADS
PRODUCT STAGE ON PROCESS USE STAGE END OF LIFE STAGE BEYOND THE
STAGE SYSTEM
BOUNDARIES
5 Environmental Product Declaration ArcelorMittal – XCarb® Recycled and Renewably Produced Hot Rolled Coils
lairetam
waR
ylppus tropsnarT
gnirutcafunaM
eht
morf
tropsnarT
etis
eht
ot
etag
ylbmessA esU
ecnanetniaM
riapeR
tnemecalpeR tnemhsibrufeR
ygrene
lanoitarepO esu
retaw
lanoitarepO esu
noitcurtsnoc-eD
noitilomed tropsnarT
gnissecorp
etsaW
lasopsiD -esueR -yrevoceR -gnilcyceR laitnetop
A1 A2 A3 A4 A5 B1 B2 B3 B4 B5 B6 B7 C1 C2 C3 C4 D
X X X MND MND MND MND MNR MNR MNR MND MND MND MND X X X
RESULTS OF THE LCA - ENVIRONMENTAL IMPACT according to EN 15804+A1: 1 ton XCarb® Recycled
and Renewably Produced Hot Rolled Coil
Parameter Unit A1-A3 C3 C4 D
Global warming potential [kg CO2-Eq.] 5.32E+2 1.50E+0 2.83E-1 -1.70E+1
Depletion potential of the stratospheric ozone layer [kg CFC11-Eq.] 1.00E-7 2.35E-11 8.25E-13 5.65E-11
Acidification potential of land and water [kg SO2-Eq.] 1.02E+0 2.95E-3 1.69E-3 -3.91E-2
Eutrophication potential [kg (PO4)3--Eq.] 9.14E-2 4.28E-4 1.88E-4 -3.24E-3
Formation potential of tropospheric ozone photochemical
[kg ethene-Eq.] 1.07E-1 2.49E-4 1.33E-4 -5.11E-3
oxidants
Abiotic depletion potential for non-fossil resources [kg Sb-Eq.] 1.63E-3 4.10E-7 3.09E-8 3.96E-7
Abiotic depletion potential for fossil resources [MJ] 5.30E+3 1.67E+1 3.78E+0 -1.33E+2
RESULTS OF THE LCA - INDICATORS TO DESCRIBE RESOURCE USE according to EN 15804+A1: 1 ton
XCarb® Recycled and Renewably Produced Hot Rolled Coil
Parameter Unit A1-A3 C3 C4 D
Renewable primary energy as energy carrier [MJ] 1.89E+4 1.39E+1 5.87E-1 1.88E+1
Renewable primary energy resources as material utilization [MJ] 0.00E+0 0.00E+0 0.00E+0 0.00E+0
Total use of renewable primary energy resources [MJ] 1.89E+4 1.39E+1 5.87E-1 1.88E+1
Non-renewable primary energy as energy carrier [MJ] 5.39E+3 2.68E+1 3.91E+0 -1.30E+2
Non-renewable primary energy as material utilization [MJ] 0.00E+0 0.00E+0 0.00E+0 0.00E+0
Total use of non-renewable primary energy resources [MJ] 5.39E+3 2.68E+1 3.91E+0 -1.30E+2
Use of secondary material [kg] 9.71E+2 0.00E+0 0.00E+0 8.80E+0
Use of renewable secondary fuels [MJ] 0.00E+0 0.00E+0 0.00E+0 0.00E+0
Use of non-renewable secondary fuels [MJ] 0.00E+0 0.00E+0 0.00E+0 0.00E+0
Use of net fresh water [m³] 2.87E+0 1.32E-2 9.93E-4 -1.13E-2
RESULTS OF THE LCA – WASTE CATEGORIES AND OUTPUT FLOWS according to EN 15804+A1:
1 ton XCarb® Recycled and Renewably Produced Hot Rolled Coil
Parameter Unit A1-A3 C3 C4 D
Hazardous waste disposed [kg] 2.40E-6 2.23E-9 2.01E-10 6.45E-9
Non-hazardous waste disposed [kg] 1.21E+1 1.90E-2 2.00E+1 -2.46E-1
Radioactive waste disposed [kg] 4.32E-3 3.95E-3 4.35E-5 2.16E-3
Components for re-use [kg] 0.00E+0 0.00E+0 0.00E+0 0.00E+0
Materials for recycling [kg] 0.00E+0 9.80E+2 0.00E+0 0.00E+0
Materials for energy recovery [kg] 0.00E+0 0.00E+0 0.00E+0 0.00E+0
Exported electrical energy [MJ] 0.00E+0 0.00E+0 0.00E+0 0.00E+0
Exported thermal energy [MJ] 0.00E+0 0.00E+0 0.00E+0 0.00E+0
Note: 971.2 kg of scrap are used in the manufacturing of 1 metric ton of XCarb® Recycled and Renewably
Produced Hot Rolled Coils. After use, 980 kg steel is recycled, and 20 kg is landfilled. The potential environmental
impact calculated for module D depends on the net amount of scrap left in the system, which is 980-971.2 = 8.8
kg. This means that the system has a net output of 8.8 kg of scrap, which is shown in module D as an
environmental credit or burden depending on the impact category.
References
EN 1993-1-3 steels - Part 1: General technical delivery conditions.
EN 1993-1-3:2006 - Eurocode 3 - Design of steel
structures - Part 1-3: General rules - Supplementary EN 10025-2
rules for cold-formed members and sheeting. EN 10025-2:2019 - Hot rolled products of structural
steels - Part 2: Technical delivery conditions for non-
EN 10025-1 alloy structural steels.
EN 10025-1:2004 - Hot rolled products of structural
EN 10025-3 European Commission Technical Steel Research
EN 10025-3:2019 - Hot rolled products of structural Sansom, M.and Meijer, J.:Life-cycle assessment (LCA)
steels - Part 3: Technical delivery conditions for for steel construction, European Commission technical
normalized/normalized rolled weldable fine grain steel research, 2001-12.
structural steels.
GaBi ts Documentation
EN 10025-4 GaBi ts dataset documentation for the GaBi datasets
EN 10025-4:2019 - Hot rolled products of structural for Life Cycle Engineering. LBP, University of Stuttgart
steels - Part 4: Technical delivery conditions for and PE International, 2011.
thermomechanical rolled weldable fine grain structural http://documentation.gabi-software.com/.
steels.
GaBi ts Software
EN 10025-5 GaBi ts Software and Databases for Life Cycle
EN 10025-5:2019 - Hot rolled products of structural Engineering. LBP, University of Stuttgart and PE
steels - Part 5: Technical delivery conditions for International, 2013.
structural steels with improved atmospheric corrosion
resistance. IBU 2021
Institut Bauen und Umwelt e.V.: General Instructions
EN 10111 for the EPD programme of Institut Bauen und Umwelt
EN 10011:2008 - Continuously hot rolled low carbon e.V., Version 2.0, Berlin: Institut Bauen und Umwelt
steel sheet and strip for cold forming. e.V., 2021.
www.ibu-epd.com
EN 10149-1
EN 10149-1:2013 - Hot rolled flat products made of PCR Part A
high yield strength steels for cold forming - Part 1: PCR - Part A: Calculation Rules for the Life Cycle
General technical delivery conditions. Assessment and Requirements on the Project Report,
version 2.1.Institut Bauen und Umwelt e.V., 2021.
EN 10149-2 www.bauumwelt.com
EN 10149-2:2013 - Hot rolled flat products made of
high yield strength steels for cold forming - Part 2: PCR Part B
Technical delivery conditions for thermomechanically PCR - Part B: Requirements of the EPD for Structural
rolled steels. steels, Institut Bauen und Umwelt e.V., 2017.
www.bauumwelt.com
EN 10149-3
EN 10149-3:2013 - Hot rolled flat products made of Candidate list - REACH
high yield strength steels for cold forming - Part 3: Regulation (EC) No 1907/2006 of the European
Technical delivery conditions for normalized or Parliament and of the Council on the Registration,
normalized rolled steels. Evaluation, Authorisation and Restriction
of Chemicals (REACH).
EN 15804 https://echa.europa.eu/candidate-list-table
EN 15804:2012+A1:2013, Sustainability of
construction works — Environmental Product Regulation (EU) No. 305/2011 (CPR)
Declarations — Core rules for the product category of Regulation of the European Parliament and of the
construction products. Council (EU) No 305/2011 of 9 March 2011 laying
down harmonized conditions for the marketing of
EN ISO 683 construction products and repealing Council Directive
EN ISO 683-1:2012 - Heat-treatable steels, alloy steels 89/106 / EEC, Official Journal EU No L 88, 4.4.2011
and free-cutting steels.
Worldsteel Association Methodology Report
ASTM G101-04(2015) Life cycle assessment (LCA) methodology report for
Standard Guide for Estimating the Atmospheric steel products.
Corrosion Resistance of Low-Alloy Steels, ASTM © World Steel Association 2017.
International, West Conshohocken, PA, 2015 https://worldsteel.org/wp-content/uploads/Life-cycle-
inventory-methodology-report.pdf
ISO 14025
EN ISO 14025:2011, Environmental labels and
declarations — Type III environmental declarations —
Principles and procedures.
6 Environmental Product Declaration ArcelorMittal – XCarb® Recycled and Renewably Produced Hot Rolled Coils
Publisher
Institut Bauen und Umwelt e.V. Tel +49 (0)30 3087748- 0
Hegelplatz 1 Fax +49 (0)30 3087748- 29
10117 Berlin Mail info@ibu-epd.com
Germany Web www.ibu-epd.com
Programme holder
Institut Bauen und Umwelt e.V. Tel +49 (0)30 - 3087748- 0
Hegelplatz 1 Fax +49 (0)30 – 3087748 - 29
10117 Berlin Mail info@ibu-epd.com
Germany Web www.ibu-epd.com
Author of the Life Cycle
Assessment Tel +352 4792-1
ArcelorMittal Europe – Flat Fax -
Products Mail
Boulevard d’Avranches 24-26 flateurope.technical.assistance@
1160 Luxembourg arcelormittal.com
Luxembourg Web flateurope.arcelormittal.com/
Owner of the Declaration
ArcelorMittal Europe – Flat Tel +352 4792-1
Products Fax -
Boulevard d’Avranches 24-26 Mail
1160 Luxembourg flateurope.technical.assistance@
Luxembourg arcelormittal.com
Web flateurope.arcelormittal.com/
