ENVIRONMENTAL PRODUCT DECLARATION
as per ISO 14025 and EN 15804+A2
Owner of the Declaration Halbmond Teppichwerke GmbH
Publisher Institut Bauen und Umwelt e.V. (IBU)
Programme holder Institut Bauen und Umwelt e.V. (IBU)
Declaration number EPD-HBM-20230143-CBC1-EN
Issue date 05.05.2023
Valid to 04.05.2028
Tufted wall-to-wall carpet with a pile material of PA 6 Econyl® with
100% recycled content and a felt backing of 600 g/m2 PET
Halbmond Teppichwerke GmbH
www.ibu-epd.com | https://epd-online.com
General Information
Halbmond Teppichwerke GmbH Tufted wall-to-wall carpet with a pile material of PA
6 Econyl® with 100% recycled content and a felt
backing of 600 g/m2 PET
Programme holder Owner of the declaration
IBU – Institut Bauen und Umwelt e.V. Halbmond Teppichwerke GmbH
Hegelplatz 1 Brückenstraße 1
10117 Berlin 08606 Oelsnitz
Germany Germany
Declaration number Declared product / declared unit
EPD-HBM-20230143-CBC1-EN Tufted wall-to-wall carpet with a pile material of PA 6 with 100% recycled
content and a felt backing of 600 g/m2 PET with 99.6% recycled content
This declaration is based on the product category rules: Scope:
Floor coverings, 01.08.2021 The manufacturer declaration applies to tufted wall-to-wall carpet with a
(PCR checked and approved by the SVR) PET felt backing, a pile material of PA 6 with 100% recycled content and a
maximum total pile weight of 745 g/m2. The products are produced in
Oelsnitz/Vogtl., Germany.
Issue date The owner of the declaration shall be liable for the underlying information
and evidence; the IBU shall not be liable with respect to manufacturer
05.05.2023
information, life cycle assessment data and evidences.
The EPD was created according to the specifications of EN 15804+A2. In
Valid to
the following, the standard will be simplified as EN 15804.
04.05.2028
Verification
The standard EN 15804 serves as the core PCR
Independent verification of the declaration and data according to ISO
14025:2011
internally X externally
Dipl.-Ing. Hans Peters
(Chairman of Institut Bauen und Umwelt e.V.)
Florian Pronold Angela Schindler,
(Managing Director Institut Bauen und Umwelt e.V.) (Independent verifier)
Environmental Product Declaration - Halbmond Teppichwerke GmbH - Tufted wall-to-wall carpet with a pile material of PA 6 Econyl® with 100% recycled content and a
1 felt backing of 600 g/m2 PET
Product
characteristics according to EN 14041: 2018-05, Resilient,
Product description/Product definition textile and laminate floor coverings - Essential characteristics.
The declaration applies to tufted wall-to-wall carpets having a Additional product properties in accordance with EN 1307 can
surface pile of 100% recycled solution dyed polyamide 6 with a be found on the Product Information System PRODIS using the
maximum total pile weight of 745 g/m2. The backing of the PRODIS registration number of the product (www.pro-dis.info)
carpet consists of a felt backing of 600 g/m2 PET with 99.6% or on the manufacturer's technical information section.
recycled content. The total recycled content of the carpet is
Base materials/Ancillary materials
57%. The chromojet printing system allows the creation of
various designs. For the placing on the market of the specific Name Value Unit
product in the European Union/European Free Trade Polyamide 6 32.7 %
Association (EU/EFTA) (with the exception of Switzerland)
Polyester 29.2 %
Regulation (EU) No. 305/2011 Construction Product Regulation
SBR Latex 13.9 %
(CPR) applies. The product needs a Declaration of
Limestone 13.0 %
Performance (DoP) taking into consideration EN 14041:2018-
05, Resilient, textile and laminate floor coverings - Essential Aluminium Hydroxide 10.3 %
characteristics, and the CE-marking. The DoP of the product Additives 0.9 %
can be found on the manufacturer's technical information
The specific product covered by the EPD contains substances
section. For the application and use of the product the
listed in the ECHA candidate list (17.01.2023) or other
respective national provisions apply.
carcinogenic, mutagenic or reprotoxic (CMR) substances in
Application categories 1A or 1B which are not on the candidate list
exceeding 0.1 percentage by mass: no
The use class of the specific product as defined in EN 1307 can
The products are registered in the GUT-PRODIS Information
be found in the Product Information System (PRODIS) using
System. The PRODIS system ensures the compliance with
the PRODIS registration number of the product.
limitations of various chemicals and Volatile Organic Compound
Technical Data (VOC)-emissions and a ban on the use of all substances that
are listed as 'Substances of Very High Concern' (SVHC) under
REACH.
Constructional data according to EN 1307
Name Value Unit Reference service life
Product Form Wall-to-wall carpet on rolls - The service life of textile floor coverings strongly depends on
the correct installation taking into account the declared use
Type of manufacture Tufted carpet -
classification and the adherence to cleaning and maintenance
Yarn type PA 6 with 100% recycled content -
instructions.
Total carpet weight 2365 g/m2 A calculation of the reference service life according to ISO
Secondary backing PET felt backing - 15686 is not possible. Alternatively, a reference service life of
Total pile weight 745 g/m2 10 years can be assumed, during which the functional and
visual quality is guaranteed (BNB, Nutzungsdauer von
Performance data of the product in accordance with the Bauteilen). The technical service life can be significantly longer.
declaration of performance with respect to its essential
LCA: Calculation rules
1 - landfill disposal
Declared Unit 2 - municipal waste incineration
3 - recovery in a cement plant
Name Value Unit
Declared unit 1 m2 A1-A3 Production:
Energy supply and production of the basic material, processing
Grammage 2.365 kg/m2
of secondary material, auxiliary material, transport of the
The declared unit refers to 1 m2 produced textile floor covering. material to the manufacturing site, emissions, waste water
The Output of module A5 'Assembly' is 1 m2 installed textile treatment, packaging material and waste processing up to the
floor covering. landfill disposal of residual waste (except radioactive waste).
The layer thickness of the specific product covered by the EPD Benefits for generated electricity and steam due to the
can be found on the Product Information System PRODIS using incineration of production waste are aggregated. Biogenic
the PRODIS registration number of the product (www.pro- carbon that is stored in renewable material (packaging paper) is
dis.info) or on the manufacturer's technical information section. taken into account as well as the associated carbon dioxide
uptake from the air from which this biogenic carbon comes.
A4 Transport:
System boundary Transport of the packed textile floor covering from factory gate
Type of EPD: to the place of installation.
Cradle-to-gate with options, module C1-C4, module D, and
additional modules A4, A5, B1, B2. A5 Installation:
System boundaries of modules A, B, C, D: Installation of the textile floor covering, processing of
Modules C3, C4 and D are indicated separately for three end- installation waste and packaging waste up to the landfill
of-life scenarios: disposal of residual waste (except radioactive waste), the
Environmental Product Declaration - Halbmond Teppichwerke GmbH - Tufted wall-to-wall carpet with a pile material of PA 6 Econyl® with 100% recycled content and a
2 felt backing of 600 g/m2 PET
production of the amount of carpet that occurs as installation C3-2: Impact from waste incineration (plant with R1>0.6),
waste including its transport to the place of installation. generated electricity and steam are listed in the result table as
Generated electricity and steam due to the incineration of exported energy.
waste are listed in the result table as exported energy. Biogenic C3-3: Collection of the carpet waste for recovery in the cement
carbon that is stored in renewable materials in packaging paper industry,
is released as carbon dioxide emissions into the air at the end waste processing (granulating), transport to the cement plant,
of life in module A5. Preparation of the floor and auxiliary emissions
materials (adhesives, fixing agents, PET connectors) are from the incineration.
beyond the system boundaries and not taken into account.
C4 Disposal
B1 Use: C4-1: Impact from landfill disposal,
Indoor emissions during the use stage. After the first year, no C4-2: The carpet waste leaves the system in
product-related Volatile Organic Compound (VOC) emissions module C3-2,
are relevant due to known VOC decay curves of the product. C4-3: The pre-processed carpet waste leaves the system in
module C3-3.
B2 Maintenance:
Cleaning of the textile floor covering for a period of 1 year: D Recycling potential:
Vacuum cleaning – electricity supply Calculated benefits result from materials exclusive secondary
Wet cleaning – electricity, water consumption, production of the materials (net materials).
cleaning agent, waste water treatment. D-A5: Benefits for generated energy due to incineration of
The declared values in this module have to be multiplied by the packaging and installation waste (incineration plant with R1 >
assumed service life of the floor covering in the building in 0.6),
question. D-1: Benefits for generated energy due to landfill disposal of
carpet waste at the end-of-life,
B3 - B5: D-2: Benefits for generated energy due to incineration of carpet
The modules are not relevant within the assumed reference waste at the end-of-life (incineration plant with R1 > 0.6),
service life of 10 years. D-3: Benefits for saved fossil energy and saved inorganic
material due to recovery of the carpet in a cement plant.
B6 - B7:
No energy and water input are required for the operation of the Geographic Representativeness
carpet in the use stage. The modules do not cause any Land or region, in which the declared product system is
environmental impact. manufactured, used or handled at the end of the product´s
lifespan: Europe
C1 De-construction:
The floor covering is de-constructed manually and no additional
Comparability
environmental impact is caused.
Basically, a comparison or an evaluation of EPD data is only
possible if all the data sets to be compared were created
C2 Transport:
according to EN 15804 and the building context, respectively
Transport of the carpet waste to a landfill, to the municipal
the product-specific characteristics of performance, are taken
waste incineration plant (MWI) or to the waste collection facility
into account. Background data are taken from the GaBi
for recycling.
database, 2022-2. Remaining data gaps are covered by the
ecoinvent 3.7 database, 2020
C3 Waste processing:
C3-1: Landfill disposal needs no waste processing.
LCA: Scenarios and additional technical information
Name Value Unit
Characteristic product properties of biogenic carbon
Material loss 0.213 kg
Name ValueUnit Polyethylene packaging waste and installation waste are
considered to be incinerated in a municipal waste incineration
Biogenic carbon content in accompanying kg
0.013 plant. Cardboard packaging waste is going to be recycled.
packaging at factory gate C
Preparation of the floor and auxiliaries (adhesives, fixing
1 kg biogenic Carbon is equivalent to 44/12 kg of CO 2 agents, PET connectors etc.) are not taken into account.
Maintenance (B2)
The values for cleaning refer to 1 m2 floor covering per year.
Depending on the application based on ISO 10874, the
Transport to the construction site (A4) technical service life recommended by the manufacturer and
Name Value Unit the anticipated strain on the floor by customers, the case-
Litres of fuel (truck, EURO 0-6 mix) 0.0055 l/100km specific useful life can be established. Based on this useful life
the effects of module B2 need to be calculated in order to
Transport distance 700 km
obtain the overall environmental impacts.
Capacity utilisation (including empty runs) 55 %
Installation in the building (A5)
Environmental Product Declaration - Halbmond Teppichwerke GmbH - Tufted wall-to-wall carpet with a pile material of PA 6 Econyl® with 100% recycled content and a
3 felt backing of 600 g/m2 PET
Name Value Unit Each scenario is calculated as a 100% scenario.
Scenario 1: 100 % landfill disposal
Maintenance cycle (vacuum cleaning) 208 Number /year
Scenario 2: 100 % municipal waste incineration (MWI)
Maintenance cycle (wet cleaning) 1,5 Number /year
with R1>0.6
Water consumption (wet cleaning) 0.004 m3 Scenario 3: 100 % recovery in the cement industry
Cleaning agent (wet cleaning) 0.09 kg
Electricity consumption 0.314 kWh If combinations of these scenarios have to be calculated this
should be done according to the following scheme:
For further information on cleaning and maintenance see
EOL-impact = x % impact (Scenario 1)
www.halbmond.de
+ y % impact (Scenario 2)
+ z % impact (Scenario 3)
with x % + y % + z % = 100 %
Service life
Name Value Unit Name ValueUnit
Life Span (according to BBSR) 10 a Collected as mixed construction waste (scenario 1
2.365 kg
Corresponds to the and 2)
Declared product properties (at
specifications of EN - Collected separately waste type (scenario 3) 2.365 kg
the gate) and finishes
1307 Landfilling (scenario 1) 2.365 kg
An assumed quality of work, Conforms to the Energy recovery (scenario 2) 2.365 kg
when installed in accordance
manufacturer's - Energy recovery (scenario 3) 1.816 kg
with the manufacturer’s
instructions Recycling (scenario 3) 0.549 kg
instructions
Usage conditions, e.g. Use in areas defined by Reuse, recovery and/or recycling potentials (D), relevant
frequency of use, mechanical the use class according - scenario information
exposure to EN 1307 Recovery or recycling potentials due to the three end-of-life
scenarios (module C) are indicated separately.
Maintenance e.g. required According to the
frequency, type and quality and manufacturers -
Recycling in the cement industry (scenario 3)
replacement of components instructions
The organic material of the carpet is used as an alternative fuel
End of Life (C1-C4) in a cement kiln. It mainly substitutes for lignite (68.8 %), hard
Three different end-of-life scenarios are declared and the coal (23.6 %) and petrol coke (7.6 %). The inorganic material is
results are indicated separately in module C. substantially integrated into the cement clinker and substitutes
for original material input. VDZ e.V.
Environmental Product Declaration - Halbmond Teppichwerke GmbH - Tufted wall-to-wall carpet with a pile material of PA 6 Econyl® with 100% recycled content and a
4 felt backing of 600 g/m2 PET
LCA: Results
The LCA results refer to all declared products with a maximum total pile weight of 745 g/m2. The declared result figures in module B2
have to be multiplied by the assumed service life (in years) of the floor covering in the building under consideration. Information on non-
relevant modules: Modules B3 - B7 are not relevant during the service life of the carpet. Modules C1, C3/1, C4/2 and C4/3 cause no
additional impact (see chapter "LCA: Calculation rules" in this document). All these modules are declared and marked as 'modules not
relevant/declared'. Module C2 represents the transport for scenarios 1, 2 and 3. Column D represents module D/A5.
DESCRIPTION OF THE SYSTEM BOUNDARY (X = INCLUDED IN LCA; MND = MODULE OR INDICATOR NOT DECLARED; MNR
= MODULE NOT RELEVANT)
Benefits and
Construction loads beyond
Product stage Use stage End of life stage
process stage the system
boundaries
la ire ta m w a Ry lp p u s tro p s n a rT g n iru tc a fu n a M e h t m o rf tro p s n a rTe tis e h t o t e ta g y lb m e s s A e s U e c n a n e tn ia M ria p e R tn e m e c a lp e R tn e m h s ib ru fe R y g re n e la n o ita re p Oe s u re ta w la n o ita re p Oe s u n o itc u rts n o c -e Dn o itilo m e d tro p s n a rT g n is s e c o rp e ts a W la s o p s iD -e s u e R-y re v o c e R-g n ilc y c e Rla itn e to p
A1 A2 A3 A4 A5 B1 B2 B3 B4 B5 B6 B7 C1 C2 C3 C4 D
X X X X X X X MNR MNR MNR MND MND X X X X X
RESULTS OF THE LCA - ENVIRONMENTAL IMPACT according to EN 15804+A2: 1 m² floor covering
Parameter Unit A1-A3 A4 A5 B1 B2 C1 C2 C3/2 C3/3 C4/1 D D/1 D/2 D/3
GWP-total kg CO 2 eq 6.12E+00 1.43E-01 9.9E-01 0 4.16E-01 0 8.02E-03 3.95E+003.99E+00 1.68E-01 -2.65E-02 0 -1.79E-01 -1.31E-01
GWP-fossil kg CO 2 eq 6.05E+00 1.4E-01 9.36E-01 0 2.15E-01 0 7.88E-03 3.95E+003.99E+00 1.68E-01 -2.63E-02 0 -1.78E-01 -1.31E-01
GWP-
biogenic kg CO 2 eq 6.14E-02 1.81E-03 5.37E-02 0 4.16E-03 0 1.02E-04 3.98E-04 7.62E-04 -2.72E-08 -1.32E-04 0 -8.79E-04 -2.4E-04
GWP-luluc kg CO 2 eq 6.86E-03 7.93E-04 6.98E-04 0 1.96E-01 0 4.47E-05 6.51E-05 1.79E-04 8.16E-05 -2.83E-06 0 -1.87E-05 -7.29E-05
kg CFC11
ODP 2.21E-07 8.53E-15 1.99E-08 0 3.42E-08 0 4.8E-16 3.47E-13 5.25E-13 2.25E-13 -1.73E-13 0 -1.14E-12 -1.11E-13
eq
AP mol H+ eq 1.89E-02 8.48E-04 2.11E-03 0 8.32E-04 0 4.75E-05 3.62E-03 3.77E-03 4.97E-04 -3.4E-05 0 -2.27E-04 -6.07E-04
EP-
kg P eq 4.82E-04 4.25E-07 4.35E-05 0 5.19E-06 0 2.39E-08 2.84E-07 3.79E-07 3.12E-05 -3.52E-08 0 -2.33E-07 -1.6E-07
freshwater
EP-marine kg N eq 6.11E-03 4.16E-04 7.5E-04 0 1.97E-04 0 2.34E-05 1.79E-03 1.85E-03 1.1E-04 -9.32E-06 0 -6.25E-05 -1.71E-04
EP-terrestrial mol N eq 5.7E-02 4.61E-03 7.38E-03 0 2.83E-03 0 2.6E-04 2.01E-02 2.08E-02 1.21E-03 -9.98E-05 0 -6.69E-04 -1.87E-03
kg
POCP NMVOC 1.52E-02 7.86E-04 1.85E-03 4.18E-04 9.83E-04 0 4.42E-05 4.57E-03 4.7E-03 3.52E-04 -2.61E-05 0 -1.75E-04 -4.96E-04
eq
ADPE kg Sb eq 3.46E-05 1.19E-08 3.11E-06 0 2.3E-07 0 6.69E-10 1.33E-08 1.83E-08 1.16E-08 -3.9E-09 0 -2.59E-08 -1.36E-08
-3.02E -9.68E
ADPF MJ 1E+02 1.9E+00 9.35E+00 0 5.9E+00 0 1.07E-01 1.65E+002.14E+00 2.39E+00 -4.48E-01 0
+00 +00
m3 world
WDP eq 5.27E+00 1.27E-03 5.17E-01 0 9.99E-02 0 7.17E-05 4.46E-01 4.49E-01 -1.78E-03 -2.7E-03 0 -1.78E-02 -1.68E-02
deprived
GWP = Global warming potential; ODP = Depletion potential of the stratospheric ozone layer; AP = Acidification potential of land and water; EP =
Eutrophication potential; POCP = Formation potential of tropospheric ozone photochemical oxidants; ADPE = Abiotic depletion potential for non-fossil
resources; ADPF = Abiotic depletion potential for fossil resources; WDP = Water (user) deprivation potential)
RESULTS OF THE LCA - INDICATORS TO DESCRIBE RESOURCE USE according to EN 15804+A2: 1 m² floor covering
Parameter Unit A1-A3 A4 A5 B1 B2 C1 C2 C3/2 C3/3 C4/1 D D/1 D/2 D/3
PERE MJ 4.89E+01 1.08E-01 4.5E+00 0 3.68E+00 0 6.08E-03 2.71E-01 4.08E-01 1.96E-01 -1.2E-01 0 -7.87E-01 -2.27E-01
PERM MJ 5.9E-02 0 -5.9E-02 0 0 0 0 0 0 0 0 0 0 0
PERT MJ 4.89E+01 1.08E-01 4.44E+00 0 3.68E+00 0 6.08E-03 2.71E-01 4.08E-01 1.96E-01 -1.2E-01 0 -7.87E-01 -2.27E-01
PENRE MJ 9.05E+011.91E+00 9.67E+00 0 5.9E+00 0 1.07E-01 1.15E+01 1.2E+01 2.39E+00 -4.48E-01 0 -3.02E+00-9.69E+00
-9.82E -9.82E
PENRM MJ 1.01E+01 0 -3.01E-01 0 0 0 0 0 0 0 0 0
+00 +00
PENRT MJ 1E+02 1.91E+00 9.36E+00 0 5.9E+00 0 1.07E-01 1.66E+00 2.15E+00 2.39E+00 -4.48E-01 0 -3.02E+00-9.69E+00
SM kg 1.47E+00 0 1.33E-01 0 0 0 0 0 0 0 0 0 0 3.33E-01
RSF MJ 0 0 0 0 0 0 0 0 0 0 0 0 0 0
NRSF MJ 0 0 0 0 0 0 0 0 0 0 0 0 0 0
FW m3 1.3E-01 1.22E-04 1.27E-02 0 3.34E-03 0 6.88E-06 1.05E-02 1.07E-02 2.79E-05 -1.14E-04 0 -7.52E-04 -1.04E-03
PERE = Use of renewable primary energy excluding renewable primary energy resources used as raw materials; PERM = Use of renewable primary
energy resources used as raw materials; PERT = Total use of renewable primary energy resources; PENRE = Use of non-renewable primary energy
excluding non-renewable primary energy resources used as raw materials; PENRM = Use of non-renewable primary energy resources used as raw
materials; PENRT = Total use of non-renewable primary energy resources; SM = Use of secondary material; RSF = Use of renewable secondary fuels;
NRSF = Use of non-renewable secondary fuels; FW = Use of net fresh water
RESULTS OF THE LCA – WASTE CATEGORIES AND OUTPUT FLOWS according to EN 15804+A2:
1 m² floor covering
Environmental Product Declaration - Halbmond Teppichwerke GmbH - Tufted wall-to-wall carpet with a pile material of PA 6 Econyl® with 100% recycled content and a
5 felt backing of 600 g/m2 PET
Parameter Unit A1-A3 A4 A5 B1 B2 C1 C2 C3/2 C3/3 C4/1 D D/1 D/2 D/3
HWD kg 2.25E-03 9.13E-12 2.02E-04 0 4.19E-05 0 5.13E-13 2.46E-10 2.66E-10 3.67E-10 -6.12E-11 0 -4.16E-10 -1.67E-10
NHWD kg 4.96E-01 2.74E-04 7.4E-02 0 7.3E-03 0 1.54E-05 3.24E-01 3.24E-01 2.36E+00 -2.23E-04 0 -1.49E-03 -1.15E-01
RWD kg 3.29E-03 2.35E-06 3.02E-04 0 3.76E-04 0 1.32E-07 5.97E-05 9.51E-05 2.93E-05 -3.42E-05 0 -2.26E-04 -5.18E-05
CRU kg 0 0 0 0 0 0 0 0 0 0 0 0 0 0
MFR kg 0 0 3E-02 0 0 0 0 0 3.33E-01 0 0 0 0 0
MER kg 0 0 0 0 0 0 0 0 0 0 0 0 0 0
EEE MJ 0 0 6.07E-01 0 0 0 0 6.22E+00 0 0 0 0 0 0
EET MJ 0 0 1.1E+00 0 0 0 0 1.13E+01 4.73E+01 0 0 0 0 0
HWD = Hazardous waste disposed; NHWD = Non-hazardous waste disposed; RWD = Radioactive waste disposed; CRU = Components for re-use;
MFR = Materials for recycling; MER = Materials for energy recovery; EEE = Exported electrical energy; EET = Exported thermal energy
RESULTS OF THE LCA – additional impact categories according to EN 15804+A2-optional:
1 m² floor covering
Parameter Unit A1-A3 A4 A5 B1 B2 C1 C2 C3/2 C3/3 C4/1 D D/1 D/2 D/3
Disease
PM 1.38E-07 4.9E-09 1.4E-08 0 6.84E-08 0 2.75E-10 1.23E-08 1.32E-08 4.78E-09 -2.82E-10 0 -1.88E-09 -1.11E-08
incidence
kBq U235
IR 6.43E-01 3.44E-04 5.87E-02 0 6.78E-02 0 1.94E-05 9.24E-03 1.52E-02 4.31E-03 -5.8E-03 0 -3.82E-02 -6.99E-03
eq
ETP-fw CTUe 6.88E+011.32E+006.38E+00 0 2.69E+00 0 7.43E-02 6.85E-01 9.66E-01 2.33E+00 -9.56E-02 0 -6.3E-01 -2E+00
HTP-c CTUh 3.27E-09 2.67E-11 3.01E-10 0 6.21E-10 0 1.5E-12 4.02E-11 4.68E-11 1.05E-10 -4.48E-12 0 -3.01E-11 -3.89E-11
HTP-nc CTUh 1.36E-07 1.58E-09 1.26E-08 0 9.46E-09 0 8.9E-11 2.35E-09 2.67E-09 8.76E-09 -1.72E-10 0 -1.16E-09 -2.73E-09
SQP SQP ND ND ND ND ND ND ND ND ND ND ND ND ND ND
PM = Potential incidence of disease due to PM emissions; IR = Potential Human exposure efficiency relative to U235; ETP-fw = Potential comparative
Toxic Unit for ecosystems; HTP-c = Potential comparative Toxic Unit for humans (cancerogenic); HTP-nc = Potential comparative Toxic Unit for humans
(not cancerogenic); SQP = Potential soil quality index
No substantiated values can be given for the SQP indicator with the existing database.
The result figures given in module B2 refer to a period of 1 year because a reference service life is not declared. They have to be
multiplied by the assumed service life (in years) of the floor covering in the building under consideration.
Disclaimer 1 – for the indicator 'Potential Human exposure efficiency relative to U235'. This impact category deals mainly with the
eventual impact of low dose ionizingradiation on human health of the nuclear fuel cycle. It does not consider effects due to possible
nuclear accidents, occupational exposure nor due to radioactive waste disposal in undergroundfacilities. Potential ionizing radiation
from the soil, from radon and from some construction materials is also not measured by this indicator.
Disclaimer 2 – for the indicators 'abiotic depletion potential for non-fossil resources', 'abiotic depletion potential for fossil resources',
'water (user) deprivation potential, deprivation-weighted water consumption', 'potential comparative toxic unit for ecosystems', 'potential
comparative toxic unit for humans – cancerogenic', 'Potential comparative toxic unit for humans - not cancerogenic', 'potential soil
quality index'.
The results of this environmental impact indicator shall be used with care as the uncertainties on these results are high or as there is
limited experienced with the indicator.
References
EN 1307 ISO 10874
DIN EN 1307: 2014+A1:2016+A2:2018-05: Textile floor DIN EN ISO 10874: 2012+A1:2021-04: Resilient, textile and
coverings - Classification laminate floor coverings - Classification
EN 13501-1 ISO 14025
DIN EN 13501-1:2019-05: Fire classification of construction DIN EN /ISO 14025:2011-10/, Environmental labels and
products and building elements - Part 1: Classification using declarations — Type III environmental declarations —
data from reaction to fire tests Principles and procedures
EN 14041 ISO 14040
DIN EN 14041: 2018-05 and DIN EN 14041: 2008-05: DIN EN ISO 14040:2006+A1:2020 Environmental
Resilient, textile and laminate floor coverings - Essential management - Life cycle assessment - Principles and
characteristics framework
EN 15804 ISO 14044
DIN EN 15804:2012+A2:2019 + AC:2021, Sustainability of DIN EN ISO 14044:2006+A1:2018+A2:2020 Environmental
construction works — Environmental Product Declarations — management - Life cycle assessment - Requirements and
Core rules for the product category of construction products guidelines
EN 16810 ISO 15686
DIN EN 16810: 2017-08: Resilient, textile and laminate floor ISO 15686: Buildings and constructed assets - Service life
coverings – Environmental product declarations – Product planning ISO 15686-1: 2011-05: Part 1: General principles and
category rules framework ISO 15686-2: 2012-05: Part 2: Service life prediction
procedures ISO 15686-7: 2017-04: Part 7: Performance
Environmental Product Declaration - Halbmond Teppichwerke GmbH - Tufted wall-to-wall carpet with a pile material of PA 6 Econyl® with 100% recycled content and a
6 felt backing of 600 g/m2 PET
evaluation for feedback of service life data from practice ISO GaBi Software-System and Database for Life Cycle
15686-8: 2008-06: Part 8: Reference service life and service- Engineering, thinkstep AG, Leinfelden-Echterdingen, 2022-2
life estimation
PCR Part A
Regulation (EU) No. 305/2011 Product Category Rules for Building-Related Products and
Regulation No. 305/2011 Construction Products Regulation Services Part A: Calculation Rules for the Life Cycle
(CPR) of the European Council and of the European Assessment and Requirements on the Project Report according
Parliament, April 2011 to EN 15804+A2:2019, V1.3, Berlin: Institut Bauen und Umwelt
e.V. (IBU), August 2022
General Instructions for the IBU-EPD Program
General Instructions for the EPD-Program of the Institut Bauen PCR Part B
und Umwelt e.V., The Preparation of Environmental Product Product Category Rules for Building-Related Products and
Declarations - EPDs, version 2.0, Institut Bauen und Umwelt Services Part B: Requirements on the EPD for floor coverings,
e.V., Berlin, January 2021, www.ibu-epd.de v1.0, Berlin: Institut Bauen und Umwelt e.V. (IBU), April 2023
BNB, Nutzungsdauer von Bauteilen PRODIS
Bewertungssystem Nachhaltiges Bauen (BNB), Nutzungsdauer Product Information System (PRODIS) of the European Carpet
von Bauteilen, Bundesministerium des Inneren, für Bau und Industry, Gemeinschaft umweltfreundlicher Teppichboden e.V
Heimat, 24.02.2017 (GUT) and European Carpet and Rug Association (ECRA),
http://www.pro-dis.info
ECHA candidate list
Candidate List of substances of very high concern (SVHCs) for REACH
authorisation, 17.01.2023, European Chemicals Agency Regulation (EC) No 1907/2006 of the European Parliament and
(ECHA), Helsinki, Finland of the Council of 18 December 2006 concerning the
Registration, Evaluation, Authorisation and Restriction of
ecoinvent Chemicals (REACH), June 2017, last update: 17.01.2023
ecoinvent, Zurich, Switzerland, database version 3.7, published
September 2020 VDZ e.V.
Association of German Cement Works, Ed. Environ-mental
GaBi database Data of the German Cement Industry 2020
Environmental Product Declaration - Halbmond Teppichwerke GmbH - Tufted wall-to-wall carpet with a pile material of PA 6 Econyl® with 100% recycled content and a
7 felt backing of 600 g/m2 PET
Publisher
Institut Bauen und Umwelt e.V. +49 (0)30 3087748- 0
Hegelplatz 1 info@ibu-epd.com
10117 Berlin www.ibu-epd.com
Germany
Programme holder
Institut Bauen und Umwelt e.V. +49 (0)30 3087748- 0
Hegelplatz 1 info@ibu-epd.com
10117 Berlin www.ibu-epd.com
Germany
Author of the Life Cycle Assessment
Gemeinschaft umweltfreundlicher Teppichboden +49 (0)241 96843 410
(GUT) e.V. mail@gut-ev.de
Schönebergstraße 2 www.gut-ev.org
52068 Aachen
Germany
Owner of the Declaration
Halbmond Teppichwerke GmbH +49 (0)37421 420
Brückenstraße 1 info@halbmond.de
08606 Oelsnitz www.halbmond.de
Germany
Environmental Product Declaration - Halbmond Teppichwerke GmbH - Tufted wall-to-wall carpet with a pile material of PA 6 Econyl® with 100% recycled content and a
8 felt backing of 600 g/m2 PET
