ENVIRONMENTAL PRODUCT DECLARATION
as per ISO 14025 and EN 15804+A1
Owner of the Declaration Etex Building Performance International
Programme holder Institut Bauen und Umwelt e.V. (IBU)
Publisher Institut Bauen und Umwelt e.V. (IBU)
Declaration number EPD-ETE-20210277-IBC1-EN
Issue date 09.12.2021
Valid to 08.12.2026
Duripanel B1
Etex Germany Exteriors GmbH
www.ibu-epd.com | https://epd-online.com
Umwelt Produktdeklaration Name des Herstellers – Name des Produkts
1. General Information
Etex Germany Exteriors GmbH Duripanel B1
Programme holder Owner of the declaration
IBU – Institut Bauen und Umwelt e.V. Etex Building Performance International
Panoramastr. 1 500 rue Marcel Demonque
10178 Berlin 84915 Avignon Cedex 9
Germany FRANCE
Declaration number Declared product / declared unit
EPD-ETE-20210277-IBC1-EN 1m² Duripanel B1 with thickness 20mm.
This declaration is based on the product Scope:
category rules:
Wood cement - Mineral-bonded wooden composites, The life cycle assessment is based on production data
01.2019 of Duripanel B1 of the year 2018 at the production site
(PCR checked and approved by the SVR) of Etex Germany Exteriors GmbH in Beckum,
Germany.
Issue date The results of the life cycle assessment provided in this
09.12.2021 EPD are based on a thickness of 20mm and are
globally valid.
Valid to The LCA results for additional thicknesses are
declared in an annexe to this EPD.
08.12.2026
The owner of the declaration shall be liable for the
underlying information and evidence; the IBU shall not
be liable with respect to manufacturer information, life
cycle assessment data and evidences.
The EPD was created according to the specifications
of EN 15804+A1. In the following, the standard will be
simplified as EN 15804.
Verification
The standard EN 15804 serves as the core PCR
Independent verification of the declaration and data
according to ISO 14025:2010
Dipl. Ing. Hans Peters internally x externally
(chairman of Institut Bauen und Umwelt e.V.)
Dr. Alexander Röder Dipl. Natw. ETH Sascha Iqbal
(Managing Director Institut Bauen und Umwelt e.V.)) (Independent verifier)
2. Product
2.1 Product description/Product definition consideration EN 13986: 2015, Wood-based panels for
Duripanel B1 is a three-layer cement-bonded use in construction - Characteristics, evaluation of
particleboard according to EN 634-1 and -2 for internal conformity and marking and the CE-marking.
and external construction applications. It mainly For the application and use the respective national
consists of the natural raw material wood particles and provisions apply.
cement.
It is being produced in different thicknesses between 8 2.2 Application
and 40 mm. It is available in an unsanded smooth or The Duripanel B1 base panel with straight edges can
sanded surface, with smooth trimmed edges or with be used in timber frame construction, high-quality
tongue and groove. The surface colour is mainly being interior finishing and container construction as a load-
characterized by the fine wood particles in the outside bearing and stiffening wood-based panel.
layers. The Duripanel B1 installation panels with tongue and
groove can be used for supporting formwork and dry
For the placing on the market of the product in the subfloors with high compressive strength.
European Union/European Free Trade Association
(EU/EFTA) (with the exception of Switzerland) 2.3 Technical Data
Regulation (EU) No. 305/2011 (CPR) applies. The
construction product is covered by the harmonized The constructional data shown in the table are valid for
declaration of performance No. Si- all thicknesses and surfaces (sanded/unsanded),
DOP/Duripanel_B1/v01.10.2020 taking into unless where indicated otherwise.
2 Environmental Product Declaration Etex Germany Exteriors GmbH – Duripanel B1
(EU) Ordinance on Biocide Products No. 528/2012):
Constructional data no.
Name Value Unit
Raw density acc. to EN 634-2; EN 2.6 Manufacture
≥ 1000 kg/m³
13986 The production of large-format panels from wood
Grammage (20 mm) 25.3 kg/m2 cement takes place according to a largely automated,
Bending strength (longitudinal) ≥ 9 N/mm2 semi-dry spreading process in which no excess water
Bending strength (transverse) ≥ 9 N/mm2 is produced. In a mechanical mixer, the litter mixture of
E-module (longitudinal) ≥ 4500 N/mm2 wood chips, cement, recycled material from trimming
E-module (transverse) ≥ 4500 N/mm2 waste, auxiliary materials and water is processed. The
Tensile strength rectangular material is evenly distributed on carrier plates via a
(internal bond) ≥ 0.5 N/mm2 mechanical throw sifting system. Excess material at
the edges is returned directly to the spreader. The
Thermal conductivity λ acc. to DIN
0.23 W/(mK) scattered material is pressed, stored in a climatic
EN 13986
chamber for setting (heat exchanger, steam generation
Water vapour diffusion resistance 40 (moist);
- via natural gas), the hardened sheets restacked,
factor µ acc. to DIN EN ISO 12572 67 (dry)
trimmed and temporarily stored for 28 days. The
Moisture content at 23 °C, 80%
9 Vol. % panels are then dried in a circulating air oven to the
acc. to DIN EN ISO 12571
moisture content required for delivery.
Coefficient of thermal expansion
11 10-6K-1
αt
The quality management system of the company and
Swelling in thickness 24h acc. to
≤ 1,5 % the production facility are certified according to ISO
EN 634-2
9001.
Sound absorption coefficient (only 10 at 250-
with reference to the 500Hz / 30
% 2.7 Environment and health during
corresponding component design) at 1000-
manufacturing
acc. to EN 13986 2000Hz
During the entire manufacturing process, no health and
safety measures are required beyond the legally
stipulated occupational health and safety measures for
For more detailed info on product characteristics
commercial enterprises.
please refer to the latest DOP.
Air: Any dust produced is collected in filter systems
The performance data of the product is in accordance
and partially recycled. The emissions are well below
with the declaration of performance with respect to its
the limit values of TA Luft.
essential characteristics according to the standards
mentioned in the headline in the table for
Water/Soil: The water resulting from production and
constructional data.
plant cleaning is mechanically clarified in wastewater
treatment plants on the factory premises and reused in
the production process.
2.4 Delivery status
Duripanel B1 basic panels are available in two sizes
Noise: Noise emissions from production plants to the
1250 x 2600 mm or 1250 x 3100 mm.
environment are below the permissible limits.
The panels are delivered sanded and unsanded in
various thicknesses:
The environmental management system of the
8, 10, 12, 14, 16, 18, 20, 22, 24, 28, 32, 36, 40 mm.
company and the production facility are certified ISO
14001.
Duripanel B1 installation panels are available in sizes
1250 x 625 mm. The panels are delivered sanded on
2.8 Product processing/Installation
both sides in thicknesses 18 and 25 mm.
The processing of Duripanel can include the following
processes, for example: sawing, drilling, grinding.
2.5 Base materials/Ancillary materials
Under certain conditions Duripanel can be milled.
The main raw materials used are (in weight
percentages; dry) :
Fixing the boards will require appropriate means,
- 55-75% Portland cement
which will depend upon the application and bearing
- 15-25% spruce wood (Atro)
structure. Boards can be installed using screws or
- 5-15% recycled production residues
glues. Under certain conditions, the boards can be
fixed using clamps.
By using cement as a binder, no binder related
When selecting structurally necessary additional
isocyanates, synthetic resin or formaldehyde are being
products, care must be taken that these do not
added. No wood protection agents are being used.
adversely affect the described properties of the
environmental compatibility of the construction
This article contains substances listed in the candidate
products mentioned.
list (date: 08.07.2021) exceeding 0.1 percentage by
mass: no.
The local regulations for the workers’ health and safety
This article contains other carcinogenic, mutagenic,
and the environment apply (e.g. trade associations or
reprotoxic (CMR) substances in categories 1A or 1B
ordinance on hazardous substances). Also, when
which are not on the candidate list, exceeding 0.1
processing the above-mentioned products, the usual
percentage by mass: no.
occupational health and safety measures must be
Biocide products were added to this construction
observed in accordance with the manufacturer's
product or it has been treated with biocide products
instructions. It should be noted that dust produced
(this then concerns a treated product as defined by the
during processing can react alkaline (pH value: approx.
3 Environmental Product Declaration Etex Germany Exteriors GmbH – Duripanel B1
12). The machining tools and equipment used at the Smoke gas development - base panel s1
workplace should be such that the relevant dust limits Burning droplets - base panel d0
are observed. Building material class - installation panel Bfl
For example, in Germany the general dust limit value Smoke gas development - installation panel s1
is given in the directive TRGS 900. According to Burning droplets - installlation panel -
current knowledge, water, air and soil cannot be
endangered if wood cement is processed as intended. Water
No ingredients that could be hazardous to water are
2.9 Packaging
washed out (see also item Evidence: Eluate analysis).
PE shrink films, paper, wooden pallets and steel
The pH value is basic (pH ≥ 12).
strapping are used as packaging materials. The
wooden pallets used are one-way pallets. Mechanical destruction
Extraordinary effects related to a mechanical
destruction (e.g. emissions) are not known.
2.10 Condition of use
Duripanel building boards are resistant to the effects of 2.14 Re-use phase
moisture and are not physically affected when used in Several possibilities exist for the boards after the end-
humid or wet conditions. Some performance of-life of the application in which they were used.
characteristics are affected by moisture content. The
panels do not promote mould growth and are resistant In undamaged form, the dismantled products can be
to attacks by insects or vermin. used again in accordance with their original purpose
or, for example, be reused as foundation wall
Setting (hydration) of the cement-water mixture
protection.
produces hardened cement paste (calcium silicate If not contaminated with other building construction
hydrates) with embedded wood chips, ground
material, the boards can be ground up again and
production waste and auxiliary materials, with the reused as an additive in the production of wood
proportions indicated in the item 2.5 "Base materials".
cement (material recycling).
Over the period of use, free lime from the cement
reacts with carbon dioxide from the air to form calcium Furthermore, the products referred to could be used as
carbonate (carbonation). filler and bulk material in civil engineering, road
construction or e.g. for noise barriers (material
Wood cement contains approx. 9-11 % water
recycling).
(equilibrium moisture) which can vary with the
environmental conditions. In addition, material and energetic recycling in the
cement plant is possible.
2.11 Environment and health during use
Duripanel B1 is chemically inert. When the product is 2.15 Disposal
used as designed, the current state of knowledge For the consideration of possible disposal channels,
indicates that hazards to water, air and soil cannot the following disposal stages are proposed:
arise.
A) Production waste (before use)
The ingredients of the construction product are firmly B) Waste generated before use
bound in the state of use. Dust emissions will not occur a) at a finishing company that cuts panels to size
unless the boards are machined with abrasive tools. In b) during installation on the building site
case of contact (skin, eye, mouth contact), it should be C) Waste after use, when a building is demolished or
noted that hardened cement paste reacts slightly when structural changes are made during the use
alkaline in combination with moisture. phase of the building.
2.12 Reference service life Disposal channels at stage A)
The service life according to the “Bundesinstitut für If the wood cement products are separated by type in
Bau-, Stadt- und Raumforschung“ (BBSR) table the factory, they can be ground again and reused as
“Service lives of components for life cycle assessment an additive in the production of wood cement (material
according to Bewertungssystem Nachhaltiges recycling). This shall be preferred.
Bauen (BNB)" is indicated to be >50 years. Thermal treatment in residual waste treatment plants
Over the service life, free lime in the cement reacts
and cement works can be considered.
with carbon dioxide in the air to form calcium The lowest priority route may be landfill.
carbonate (carbonation). There will be no verifiable
influences on ageing when the products are applied in Disposal channels at stage B) and C)
accordance with the generally accepted rules of a) At collection: keeping cement-bonded particleboard
technology. separate from wood waste as well as from other
mineral wastes
b) Thermal treatment and/or energy recovery
2.13 Extraordinary effects c) Landfill
Fire As for disposal facilities, depending on the composition
The Duripanel B1 boards have a fire classification
and quantity of waste, thermal residual waste
according to EN 13501-1 as given in the table below. treatment plants and cement works can be considered.
As the landfill classes are being defined differently in
Fire protection
the member states, the landfill class of the respective
Name Value country applies.
Building material class - base panel B
4 Environmental Product Declaration Etex Germany Exteriors GmbH – Duripanel B1
Disposal channels B) and C) 17 09 04 (mixed
The following waste codes are suggested in construction and demolition wastes other than those
accordance with the European List of Waste: mentioned in 17 09 01, 17 09 02 and 17 09 03).
Disposal channel A) 10 13 11 (wastes from cement-
based composite materials other than those mentioned 2.16 Further information
in 10 13 09 and 10 13 10). Further information can be found on the homepage
https://www.siniat.com/.
3. LCA: Calculation rules
3.1 Declared Unit 1) Scenario 1: 100% recycling in cement plant.
The functional unit declared in this EPD is 1m² of Due to the wood content of Duripanel B1, the shredded
Duripanel B1 with a thickness of 20mm (abbreviated product can reduce the use of energy in the cement
as 1m²20mm). plant during cement clinker production.
In an annexe to this EPD, the LCA results for some Simultaneously, the other raw material components in
other existing thicknesses are declared. the wood cement boards help to reduce the use of
virgin raw materials in the cement plant. Energy and
Declared unit material credits were assigned using the substitution
Name Value Unit approach. The resulting credits from energy recovery
Declared unit 1 m² and material recycling are assigned to module D.
Gross density used in calculations
1263 kg/m3
based on 2018 average data 2) Scenario 2: 100% landfilling.
Grammage 25.3 kg/m2
Conversion factor to 1 kg (kg/m²) 25.3 - For both scenarios, the following processes were
included:
 energy consumption for deconstruction and
demolition
3.2 System boundary  transportation to disposal
Type of the EPD: cradle to grave.
 waste processing and recycling or landfilling
The following life cycle stages and modules are
of product
included:
Production stage (A1-A3):
 manufacturing of pre products and Loads and benefits beyond system boundary (D):
transportation to the manufacturing site  loads and benefits from recycling/landfilling of
 energy consumption during production production waste, packaging, installation
 recycling and disposal of production wastes losses and product waste.
 production of packaging
Construction stage (A4-A5):
3.3 Estimates and assumptions
 transportation of product to the construction
Most of the input and output influences of the Life
site
Cycle Inventory Analyses could be depicted using
 energy consumption during the installation of corresponding data from the GaBi database.
products There were no data records available for the wooden
 production of fixing material pallets, they were approximated using the solid
construction timber dataset. For well water, a worst
 disposal of installation wastes including
case scenario dataset “tap water from groundwater”
emissions of biogenic CO from the wood
2 was used. For the Duripanel product waste sent to
content
landfill, a combination of an inert waste dataset and a
 incineration/recycling of packaging materials municipal solid waste dataset was used in a ratio to
(potential benefits from energy substitution match the calorific value of the Duripanel B1 waste.
within the incineration process are declared in Bluewater consumption is taken into consideration in
the background data system. Water which is
module D) including emissions of biogenic
embedded in the product, as well as water which is
CO from renewable packaging materials
2 evaporated from the product during production, is
included in the calculations.
Use stage (B1-B7):
 efforts for the use of the product, 3.4 Cut-off criteria
maintenance and operational efforts All available data from production processes were
considered, i.e., all pre-products used, thermal energy
 modules B3, B4, B5 are declared as MNR
and electric power consumption as well as waste
(module not relevant) according to the IBU
management processes using the best available life
requirement. These modules are defined on
cycle inventory (LCI) datasets. This includes input
building level in general. flows with a contribution of less than 1% of mass or
energy.
Production of capital equipment, facilities and
End-of-life stage (C1-C4):
infrastructure required for manufacture are outside the
Two end-of-life scenarios were considered:
scope of this assessment.
5 Environmental Product Declaration Etex Germany Exteriors GmbH – Duripanel B1
3.5 Background data Thermal energy used at plant level in a cogeneration
The GaBi ts software was used to model the product unit could not be directly allocated to the product and
life cycle. The background data were sourced from the was allocated via recalculation based on consumed
GaBi database. amounts of electricity and steam.
Allocation for waste materials
3.6 Data quality The environmental burden of waste treatment of the
This study is mainly based on primary data collected installation loss and the incineration of packaging is
directly from the manufacturing site and therefore data assigned to the system in A5. The resulting credits for
quality can be assumed to be very good. thermal and electrical energy are declared in module
Background data are from the GaBi database, last D.
update was in 2020. The environmental burdens of the product at end-of-life
scenarios are assigned to C3 and C4, the resulting
3.7 Period under review credits for thermal and electrical energy are declared in
Data for the entire production period of 2018 were module D.
collected and used for this EPD.
3.9 Comparability
3.8 Allocation Basically, a comparison or an evaluation of EPD data
Allocation in background data is only possible if all the data sets to be compared
Specific information on allocation within the were created according to EN 15804 and the building
background data is given in the GaBi documentation. context, respectively the product-specific
Allocation of upstream data characteristics of performance, are taken into account.
The product receives recycled water provided by
another production line. GaBi database version 2020.1, SP40 serves as
Allocation in foreground data background database for the calculation of the life
The production process does not deliver any co- cycle assessment.
products. In module A1-A3, specific raw material,
water and transport data were available.
4. LCA: Scenarios and additional technical information
Transport to the building site (A4)
Name Value Unit
Transport distance 300 km
Capacity utilisation (including
61 %
empty runs)
Gross density of products
1263 kg/m3
transported
Reference service life
Installation into the building (A5) Name Value Unit
Name Value Unit Reference service life (according to
- a
Auxiliary galvanized steel screws 0.12 kg ISO 15686-1, -2, -7 and -8)
Electricity consumption 0.075 kWh Life Span (according to BBSR) >=50 a
Material loss 2.53 kg Life Span according to the
- a
Dust in the air 0 kg manufacturer
VOC in the air 0 kg Declared product properties (at the
- -
gate) and finishes
Use or application of the installed product (B1) see Design application parameters (if
section 2.12 "Use" instructed by the manufacturer),
No efforts and releases of substances occur during including the references to the - -
the normal (i.e. anticipated) use phase appropriate practices and application
codes
Maintenance (B2) An assumed quality of work, when
No efforts occur during maintenance. installed in accordance with the - -
Name Value Unit manufacturer’s instructions
Water consumption 0 m3 Outdoor environment, (for outdoor
Auxiliary 0 kg applications), e.g. weathering,
Other resources 0 kg pollutants, UV and wind exposure, - -
Electricity consumption 0 kWh building orientation, shading,
Other energy carriers 0 MJ temperature
Material loss 0 kg Indoor environment (for indoor
applications), e.g. temperature, - -
moisture, chemical exposure
Usage conditions, e.g. frequency of
- -
use, mechanical exposure
Maintenance e.g. required frequency,
type and quality and replacement of - -
components
6 Environmental Product Declaration Etex Germany Exteriors GmbH – Duripanel B1
Operational energy use (B6) and Operational water
use (B7)
No efforts occur in modules B6 and B7.
Name Value Unit
Water consumption 0 m3
Electricity consumption 0 kWh
Other energy carriers 0 MJ
Equipment output 0 kW
End-of-life (C1-C4)
Two end-of-life scenarios are considered :
- scenario 1: 100% recycling in cement plant
- scenario 2: 100% landfill
Name Value Unit
Collected as mixed construction
25.42 kg
waste
Recycling (scenario 1) 25.42 kg
Recycling (scenario 2) 0.12 kg
Landfilling (scenario 1) 0 kg
Landfilling (scenario 2) 25.3 kg
Reuse, recovery and/or recycling potentials (D),
relevant scenario information
Possible benefits from the recycling of production
waste and installation losses were considered. Also,
benefits from the incineration of packaging were
considered. Additionally, benefits from the recycling of
the product at the end-of-life was taken into account
according to the selected scenario.
Name Value Unit
Recycled production waste 1.38 kg
Recycled installation losses 0.884 kg
PE packaging 12.2 g
Wood packaging 524 g
Paper packaging 0.83 g
Steel strip packaging 5.56 g
EoL Recycling (scenario 1) 25.4 kg
EoL Recycling (scenario 2) 0.12 kg
7 Environmental Product Declaration Etex Germany Exteriors GmbH – Duripanel B1
5. LCA: Results
DESCRIPTION OF THE SYSTEM BOUNDARY (X = INCLUDED IN LCA; MND = MODULE NOT DECLARED;
MNR = MODULE NOT RELEVANT)
BENEFITS AND
CONSTRUCTI LOADS
PRODUCT STAGE ON PROCESS USE STAGE END OF LIFE STAGE BEYOND THE
STAGE SYSTEM
BOUNDARIES
8 Environmental Product Declaration Etex Germany Exteriors GmbH – Duripanel B1
lairetam
waR
ylppus tropsnarT
gnirutcafunaM
eht
morf
tropsnarT
etis
eht
ot
etag
ylbmessA esU
ecnanetniaM
riapeR
tnemecalpeR tnemhsibrufeR
ygrene
lanoitarepO esu
retaw
lanoitarepO esu
noitcurtsnoc-eD
noitilomed tropsnarT
gnissecorp
etsaW
lasopsiD -esueR -yrevoceR -gnilcyceR laitnetop
A1 A2 A3 A4 A5 B1 B2 B3 B4 B5 B6 B7 C1 C2 C3 C4 D
X X X X X X X MNR MNR MNR X X X X X X X
RESULTS OF THE LCA - ENVIRONMENTAL IMPACT according to EN 15804+A1: 1 m²20mm Duripanel B1
Parameter Unit A1-A3 A4 A5 B1 B2 B6 B7 C1 C2 C3/1 C3/2 C4/1 C4/2 D/1 D/2
- -
9.35E+ 3.02E+ 0.00E+ 0.00E+ 0.00E+ 0.00E+ 1.38E+ 0.00E+ 0.00E+ 7.38E+
GWP [kg CO2-Eq.]
0
5.78E-1
0 0 0 0 0
2.96E-29.46E-2
0 0 0 0
6.92E+ 1.14E+
0 0
7.35E- 1.44E- 1.18E- 0.00E+ 0.00E+ 0.00E+ 0.00E+ 8.86E- 2.35E- 4.14E- 0.00E+ 0.00E+ 2.70E- -6.56E- -1.33E-
ODP [kg CFC11-Eq.]
14 16 14 0 0 0 0 16 17 14 0 0 15 15 14
0.00E+ 0.00E+ 0.00E+ 0.00E+ 0.00E+ 0.00E+ -4.52E- -1.53E-
AP [kg SO2-Eq.] 1.80E-25.05E-42.98E-3
0 0 0 0
5.41E-58.25E-52.53E-3
0 0
3.33E-3
3 3
0.00E+ 0.00E+ 0.00E+ 0.00E+ 0.00E+ 0.00E+ -7.62E- -1.88E-
EP [kg (PO4)3--Eq.] 3.85E-39.40E-51.22E-3
0 0 0 0
6.63E-61.54E-53.10E-4
0 0
7.37E-3
4 4
-7.07E- 0.00E+ 0.00E+ 0.00E+ 0.00E+ -1.16E- 0.00E+ 0.00E+ -6.70E- -1.62E-
POCP [kg ethene-Eq.] 2.62E-3 5.59E-4 4.43E-6 2.07E-4 1.89E-3
6 0 0 0 0 6 0 0 4 4
0.00E+ 0.00E+ 0.00E+ 0.00E+ 0.00E+ 0.00E+ -4.22E- -1.74E-
ADPE [kg Sb-Eq.] 9.37E-74.77E-82.19E-5 9.24E-97.79E-94.32E-7 5.65E-8
0 0 0 0 0 0 7 7
- -
1.19E+ 7.84E+ 1.62E+ 0.00E+ 0.00E+ 0.00E+ 0.00E+ 1.28E+ 1.53E+ 0.00E+ 0.00E+ 1.00E+
ADPF [MJ] 3.28E-1 1.13E+ 1.49E+
2 0 1 0 0 0 0 0 1 0 0 1
2 1
GWP = Global warming potential; ODP = Depletion potential of the stratospheric ozone layer; AP = Acidification potential of land and water; EP =
Caption Eutrophication potential; POCP = Formation potential of tropospheric ozone photochemical oxidants; ADPE = Abiotic depletion potential for non-
fossil resources; ADPF = Abiotic depletion potential for fossil resources
RESULTS OF THE LCA - INDICATORS TO DESCRIBE RESOURCE USE according to EN 15804+A1: 1
m²20mm Duripanel B1
Parameter Unit A1-A3 A4 A5 B1 B2 B6 B7 C1 C2 C3/1 C3/2 C4/1 C4/2 D/1 D/2
PERE [MJ] 3.73E+1 4.54E-1 2.26E+10.00E+00.00E+00.00E+00.00E+0 2.35E-1 7.42E-2 1.00E+20.00E+00.00E+09.01E+1-1.91E+0-3.67E+0
PERM [MJ] 9.73E+10.00E+0-8.12E+00.00E+00.00E+00.00E+00.00E+00.00E+00.00E+0-8.91E+10.00E+00.00E+0-8.91E+10.00E+00.00E+0
PERT [MJ] 1.35E+2 4.54E-1 1.45E+10.00E+00.00E+00.00E+00.00E+0 2.35E-1 7.42E-2 1.10E+10.00E+00.00E+0 9.24E-1-1.91E+0-3.67E+0
PENRE [MJ] 1.23E+27.88E+01.77E+10.00E+00.00E+00.00E+00.00E+0 5.31E-1 1.29E+02.48E+10.00E+00.00E+01.03E+1-1.15E+2-1.81E+1
PENRM [MJ] 4.89E-1 0.00E+0-4.89E-10.00E+00.00E+00.00E+00.00E+00.00E+00.00E+00.00E+00.00E+00.00E+00.00E+00.00E+00.00E+0
PENRT [MJ] 1.23E+27.88E+01.72E+10.00E+00.00E+00.00E+00.00E+0 5.31E-1 1.29E+02.48E+10.00E+00.00E+01.03E+1-1.15E+2-1.81E+1
SM [kg] 1.66E+00.00E+0 1.66E-1 0.00E+00.00E+00.00E+00.00E+00.00E+00.00E+00.00E+00.00E+00.00E+00.00E+00.00E+00.00E+0
RSF [MJ] 0.00E+00.00E+00.00E+00.00E+00.00E+00.00E+00.00E+00.00E+00.00E+00.00E+00.00E+00.00E+00.00E+00.00E+00.00E+0
NRSF [MJ] 0.00E+00.00E+00.00E+00.00E+00.00E+00.00E+00.00E+00.00E+00.00E+00.00E+00.00E+00.00E+00.00E+00.00E+00.00E+0
FW [m³] 1.50E-2 5.29E-4 5.09E-3 0.00E+00.00E+00.00E+00.00E+0 2.72E-4 8.65E-5 1.27E-2 0.00E+00.00E+0 1.79E-3-2.38E-3-4.51E-3
PERE = Use of renewable primary energy excluding renewable primary energy resources used as raw materials; PERM = Use of
renewable primary energy resources used as raw materials; PERT = Total use of renewable primary energy resources; PENRE = Use of
non-renewable primary energy excluding non-renewable primary energy resources used as raw materials; PENRM = Use of non-
Caption
renewable primary energy resources used as raw materials; PENRT = Total use of non-renewable primary energy resources; SM = Use
of secondary material; RSF = Use of renewable secondary fuels; NRSF = Use of non-renewable secondary fuels; FW = Use of net fresh
water
RESULTS OF THE LCA – WASTE CATEGORIES AND OUTPUT FLOWS according to EN 15804+A1:
1 m²20mm Duripanel B1
Parameter Unit A1-A3 A4 A5 B1 B2 B6 B7 C1 C2 C3/1 C3/2 C4/1 C4/2 D/1 D/2
HWD [kg] 3.60E-7 3.64E-7 4.68E-8 0.00E+00.00E+00.00E+00.00E+02.20E-105.96E-8 1.03E-8 0.00E+00.00E+0 7.96E-8-6.74E-8-9.11E-9
NHWD [kg] 3.66E+0 1.25E-3 2.73E+00.00E+00.00E+00.00E+00.00E+0 3.77E-4 2.04E-4 1.76E-2 0.00E+00.00E+02.36E+1-2.99E-2-1.04E-2
RWD [kg] 1.75E-3 1.45E-5 3.86E-4 0.00E+00.00E+00.00E+00.00E+0 8.06E-5 2.37E-6 3.77E-3 0.00E+00.00E+0 1.22E-4-5.56E-4-1.27E-3
CRU [kg] 0.00E+00.00E+00.00E+00.00E+00.00E+00.00E+00.00E+00.00E+00.00E+00.00E+00.00E+00.00E+00.00E+00.00E+00.00E+0
MFR [kg] 9.79E-1 0.00E+0 1.03E-1 0.00E+00.00E+00.00E+00.00E+00.00E+00.00E+01.80E+1 9.98E-2 0.00E+00.00E+00.00E+00.00E+0
MER [kg] 4.05E-1 0.00E+0 4.05E-2 0.00E+00.00E+00.00E+00.00E+00.00E+00.00E+07.39E+00.00E+00.00E+00.00E+00.00E+00.00E+0
EEE [MJ] 2.45E-3 0.00E+01.71E+00.00E+00.00E+00.00E+00.00E+00.00E+00.00E+00.00E+00.00E+00.00E+02.63E+00.00E+00.00E+0
EET [MJ] 5.64E-3 0.00E+02.63E+00.00E+00.00E+00.00E+00.00E+00.00E+00.00E+00.00E+00.00E+00.00E+00.00E+00.00E+00.00E+0
HWD = Hazardous waste disposed; NHWD = Non-hazardous waste disposed; RWD = Radioactive waste disposed; CRU = Components
Caption for re-use; MFR = Materials for recycling; MER = Materials for energy recovery; EEE = Exported electrical energy; EET = Exported
thermal energy
6. LCA: Interpretation
Looking at the overall life cycle for the scenario 1 Within A1-A3, the pre-chains of the raw material have
(recycling), for all of the impact categories, except for the most important impact in all impact categories
ADP-elements, the product stage of Duripanel B1 except for GWP where both the raw materials and the
contributes to the largest share (>50%) to the manufacturing contribute more or less equally and
environmental performance. except for ADPE where the manufacturing contributes
the most.
The C3 phase has only minor impacts, except in the Transport of the raw materials to the production site
category ODP a relevant influence can be seen, linked (A2) has a negligible influence (<2.5%) on the overall
to the electricity use for shredding the waste material. LCA results.
Looking at the overall life cycle for the scenario 2 The LCA for Duripanel B1 is in module A1 almost fully
(landfill) in most of the impact categories (except for determined by the pre-chains of the cement.
GWP, EP and ADP-elements, the product stage of
Duripanel B1 contributes to the largest share (>50%)
to the environmental performance.
For the GWP, next to the product stage, the main
impacts occur in module C4 linked to the EOL
landfilling of the waste and re-emission of organic
carbon dioxide linked to it.
For the EP, the production waste sent to landfill in C4
is the main contributor.
7. Requisite evidence
Mo Molybdenum <0.005 mg/l
7.1 Testing pretreatment of substances used Ni Nickel 0.0465 mg/l
Measurements according to the Waste Wood Hg Mercury <0.2 mg/l
Ordinance are not relevant as no waste wood is used Se Selenium <0.002 mg/l
in the manufacture of Duripanel B1 wood cement Zn Zinc <0.0176 mg/l
products.
7.3 VOC emissions
7.2 Leaching Measurements in line with the AgBB diagram; Eurofins
Measurement in accordance with EN 71-3, University Product Testing A/S, Galten, Denmark 29.05.2008;
of Osnabrück, Institute of Chemistry, Osnabrück; report number 764160A.
03.02.2000
Results : the analysis results of the leaching of the AgBB overview of results (28 days [µg/m³])
examined boards showed that the limit values laid Name Value Unit
down in EN 71 were complied with. TVOC (C6 - C16) 160 μg/m3
Sum SVOC (C16 - C22) 0 - 5 μg/m3
Measurement in accordance with EN 12457-4, UCL R (dimensionless) 0.07 -
Umwelt Control Labor GmbH, Lünen; 23.07.2019 : VOC without NIK 16 μg/m3
Carcinogenic Substances 0 - 1 μg/m3
Name Value Unit AgBB overview of results (3 days [µg/m³])
Sb Antimony <0.001 mg/l
Name Value Unit
As Arsenic <0.001 mg/l
TVOC (C6 - C16) 540 μg/m3
Ba Barium 0.667 mg/l
Sum SVOC (C16 - C22) 0 - 5 μg/m3
Pb Lead 0.0487 mg/l
VOC without NIK 23 μg/m3
Cd Cadmium <0.0003 mg/l
Carcinogenic Substances 0 - 1 μg/m3
Cr Chromium <0.0077 mg/l
Cu Cupper 0.016 mg/l
8. References
Standards
EN ISO 14025
DIN EN 1995-1-1/NA DIN EN ISO 14025:2011-10, Environmental labels and
DIN EN 1995-1-1/NA:2013-08, National Annex – declarations — Type III environmental declarations —
Nationally determined parameters – Eurocode 5: Principles and procedures.
Design of timber structures – Part 1-1: General –
Common rules and rules for buildings. EN 12457-4
EN 12457-4:2002, Characterisation of waste.
DIN 4102-1 Leaching. Compliance test for leaching of granular
DIN 4102-1:1998, Fire behaviour of building materials waste materials and sludges. One stage batch test at a
and elements - Classification of building materials - liquid to solid ratio of 10 l/kg for materials with particle
Requirements and testing. size below 10 mm (without or with size reduction).
9 Environmental Product Declaration Etex Germany Exteriors GmbH – Duripanel B1
BBSR
EN 13501-1 BBSR table "Service lives of components for life cycle
EN 13501-1:2018, Fire classification of construction assessment according to Bewertungssystem
products and building elements - Part 1: Classification Nachhaltiges Bauen (BNB)" Sustainable Building
using data from reaction to fire tests. Information Portal by the Federal Ministry of Transport,
Building and Urban Affairs (Bundesinstitut für Bau-
EN 13986 ,Stadt-und Raumforschung, BBSR).
DIN EN 13986:2015-06, Wood-based panels for use in (https://www.nachhaltigesbauen.de/baustoff-
construction - Characteristics, evaluation of conformity undgebaeudedaten/
and marking. nutzungsdauern-von-bauteilen.html)
EN 15804 Candidate list
EN 15804:2012-04+A1 2013: Sustainability of Candidate List of substances of very high concern for
construction works — Environmental Product Authorisation, published on ECHA website, latest
Declarations — Core rules for the product category of version 08.07.2021. (https://echa.europa.eu/candidate-
construction products. list-table)
EN 1995-1-1 CPR
EN 1995-1-1:2004/A2:2014, Eurocode 5: Design of Construction Products Regulation, Regulation (EU) No
timber structures – Part 1-1: General – Common rules 305/2011 of the European Parliament and of the
and rules for buildings. Council of 9 March 2011 laying
down harmonized conditions for the marketing of
EN 634-1 construction products and repealing Council Directive
EN 634-1:1995, Cement-bonded particleboards - 89/106/ EEC Text with EEA relevance.
Specifications - Part 1: General requirements.
Eurofins Product Testing A/S
EN 634-2 Eurofins Product Testing A/S, Smedeskovvej 38, 8464
EN 634-2:2007, Cement-bonded particleboards - Galten, Denmark.
Specifications - Part 2: Requirements for OPC bonded
particleboards for use in dry, humid and external European List of Waste
conditions. 2014/955/EU: Commission Decision of 18 December
2014 amending Decision 2000/532/EC on the list of
EN 71-3 waste pursuant to Directive 2008/98/EC of the
EN 71-3:2019, Safety of toys - Part 3: Migration of European Parliament and of the Council.
certain elements. (http://data.europa.eu/eli/dec/2014/955/oj)
ISO 12571 GaBi ts software/ GaBi database
DIN EN ISO 1271:2000, Hygrothermal performance of GaBi Software System and Database for Life Cycle
building materials and products — Determination of Engineering, 1992-2020, Sphera Solutions GmbH,
hygroscopic sorption properties. Leinfelden-Echterdingen, with acknowledgement of
LBP University of Stuttgart, program version 9.5.2.49.
ISO 12572 Database version 2020.1, SP40.
DIN EN ISO 12572:2001, Hygrothermal performance
of building materials and products - Determination of GaBi documentation
water vapour transmission properties - Cup method GaBi dataset documentation for the software system
and databases, LBP, University of Stuttgart and
ISO 14025 Sphera Solutions GmbH, Leinfelden-Echterdingen,
DIN EN ISO 14025:2011-10, Environmental labels and 2020.
declarations — Type III environmental declarations — (http://www.gabi-
Principles and procedures. software.com/international/support/gabi/gabi-database-
2020-lci-documentation/)
ISO 9001
UNI EN ISO 9001:2015 September 2015, Quality
management systems - Requirements IBU 2021
Institut Bauen und Umwelt e.V.: General Programme
ISO 14001 Instructions for the Preparation of EPDs at the Institut
UNI EN ISO 14001:2015, Environmental management Bauen und Umwelt e.V. Version 2.0, Berlin: Institut
systems - Requirements with guidance for use. Bauen und Umwelt e.V., 2021. www.ibu-epd.com
OHSAS 18001 Ordinance on Biocide Products
OHSAS 18001:2007, Occupational Health and Safety Regulation (EU) No 528/2012 of the European
Management Certification. Parliament and of the Council of 22 May 2012
concerning the making available on the market and
use of biocidal products.
Further References
PCR Part A
AgBB PCR Part A: Calculation rules for the Life Cycle
Ausschuss zur gesundheitlichen Bewertung von Assessment and Requirements on the Background
Bauprodukten, AgBB (eng. German Committee for Report according to EN 15 804+A1:2013, Version
health-related evaluation of building products. 2.0.2, Institut Bauen und Umwelt e.V., 2021.
10 Environmental Product Declaration Etex Germany Exteriors GmbH – Duripanel B1
PCR Part B TRGS 900: Edition: January 2006
PCR Part B: requirements on the EPD for wood BArBl. issue 1/2006 p. 41-55
cement - mineral-bonded wooden composites, version corrected GMBl 2020 S. 276 [No. 12-13] of 30.03.2020
1.7, Institut Bauen und Umwelt e.V., 2019. amended and supplemented: GMBl 2020, 815-816
[No. 38] of 02.10.2020
REACH Regulation https://www.baua.de/DE/Angebote/Rechtstexte-und-
Regulation (EU) No 1907/2006 of the European Technische-Regeln/Regelwerk/TRGS/TRGS-900.html
Parliament and of the Council of 18 December 2006
concerning the Registration, Evaluation, Authorisation Umwelt Control Labor GmbH
and Restriction of Chemicals (REACH), establishing a Umwelt Control Labor GmbH, Postfach 2063, 44510
European Chemicals Agency, amending Directive Lünen, Deutschland.
1999/45/EC and repealing Council Regulation (EEC)
No 793/93 and Commission Waste Wood Ordinance
Regulation (EC) No 1488/94 as well as Council Ordinance on requirements for the exploitation and
Directive 76/769/EEC and Commission Directives disposal of waste wood of 15.08.2002.
91/155/EEC, 93/67/EEC, 93/105/EC and 2000/21/EC.
TA Luft
Technische Anleitung zur Reinhaltung der Luft, version
16.12.2020.
TRGS 900
11 Environmental Product Declaration Etex Germany Exteriors GmbH – Duripanel B1
Publisher
Institut Bauen und Umwelt e.V. Tel +49 (0)30 3087748- 0
Panoramastr. 1 Fax +49 (0)30 3087748- 29
10178 Berlin Mail info@ibu-epd.com
Germany Web www.ibu-epd.com
Programme holder
Institut Bauen und Umwelt e.V. Tel +49 (0)30 - 3087748- 0
Panoramastr 1 Fax +49 (0)30 – 3087748 - 29
10178 Berlin Mail info@ibu-epd.com
Germany Web www.ibu-epd.com
Author of the Life Cycle
Assessment Tel +32 (0)15 71 82 83
Peggy Van De Velde Fax +32 (0)15 71 82 29
Bormstraat 24 Mail
2830 Tisselt peggy.vandevelde@etexgroup.c
Belgium om
Web www.etexgroup.com
Owner of the Declaration
Etex Building Performance Tel +32 2 778 12 11
International Fax +32 2 778 12 12
Marcel Demonque 500 r Mail info@etexgroup.com
84915 Avignon Cedex 9 Web http://www.etexgroup.com
France
