ENVIRONMENTAL PRODUCT DECLARATION
as per ISO 14025 and EN 15804+A2
Owner of the Declaration Chemofast Anchoring GmbH
Publisher Institut Bauen und Umwelt e.V. (IBU)
Programme holder Institut Bauen und Umwelt e.V. (IBU)
Declaration number EPD-CHE-20230357-CBA4-EN
Issue date 14/09/2023
Valid to 13/09/2028
EP 1000
Chemofast Anchoring GmbH
www.ibu-epd.com | https://epd-online.com
General Information
Chemofast Anchoring GmbH EP 1000
Programme holder Owner of the declaration
IBU – Institut Bauen und Umwelt e.V. Chemofast Anchoring GmbH
Hegelplatz 1 Hanns-Martin-Schleyer-Str. 23
10117 Berlin 47877 Willich
Germany Germany
Declaration number Declared product / declared unit
EPD-CHE-20230357-CBA4-EN The declared product is the two-component reaction resin mortar "EP
1000", manufactured by Chemofast Anchoring GmbH. The declared unit is
based on 1 kg reaction resin product in the ratio at which the two
components must be mixed before use. The packaging is also included in
the calculation, since the product is sold by Chemofast with its packaging.
The declared unit is indicated in [kg].
This declaration is based on the product category rules: Scope:
Reaction resin products, 01/08/2021 This document covers the two-component reaction resin mortar "EP 1000".
(PCR checked and approved by the SVR) To prepare the life cycle assessment [LCA], specific data were collected
from the Chemofast Anchoring GmbH manufacturing facility in Willich,
Germany. The assessment is based on data from 2020 which correspond
Issue date to the yearly average.
The owner of the declaration shall be liable for the underlying information
14/09/2023
and evidence; the IBU shall not be liable with respect to manufacturer
information, life cycle assessment data and evidences.
Valid to
The EPD was created according to the specifications of EN 15804+A2. In
13/09/2028 the following, the standard will be simplified as EN 15804.
Verification
The standard EN 15804 serves as the core PCR
Independent verification of the declaration and data according to ISO
14025:2011
internally X externally
Dipl.-Ing. Hans Peters
(Chairman of Institut Bauen und Umwelt e.V.)
Florian Pronold Angela Schindler,
(Managing Director Institut Bauen und Umwelt e.V.) (Independent verifier)
1 Environmental Product Declaration - Chemofast Anchoring GmbH - EP 1000
Product
+ 10°C 1680 min.
Product description/Product definition + 15°C 1080 min.
The declared product EP 1000 is a two-component reaction + 20°C 720 min.
resin mortar based on epoxy resin that is delivered in a two- + 25°C 540 min.
component plastic cartridge. The high-performance product is + 35°C 360 min.
applied through a static mixer using a manual, battery-operated + 40°C 240 min.
or pneumatic gun. It was specially developed for use in
securing threaded rods, rebar or internally threaded sleeves in For more information, please refer to the relevant technical data
concrete. sheet.
Marketing of the product in the EU/EFTA (except for
Switzerland) is governed by Regulation (EU) No. 305/2011 Product performance values in accordance with the Declaration
(CPR). The product requires a Declaration of Performance of Performance with regard to its principal characteristics
subject to ETA-19/0201 and ETA-19/0200 and CE marking. according to ETA-19/0201 and ETA-19/0200.
Base materials/Ancillary materials
Application The declared product EP 1000 is delivered as a two-component
The EP 1000 injection system is used to safely secure threaded plastic cartridge and consists of a resin component and a
rods, internally threaded sleeves and post-mortared rebar curing agent component in a 3:1 volume ratio. The mixing ratio
connections in cracked and uncracked C20/25 to C50/60 between the resin component and the curing agent component
concrete for a useful life of up to 100 years, and is suitable for is set automatically as the
installation in hammer-drilled (standard SDS and hollow bit) and product is pushed out of the cartridge. Curing begins
diamond-drilled holes at environmental temperatures between immediately after the components are mixed.
0°C and 40°C. The EP 1000 system has ETA assessments and
ICC certifications, including seismic category C1 and C2 for 1) "This product/article/at least one partial article contains
anchoring from M8 to M30 and for rebar connections including substances in the ECHA candidate list of substances of very
seismic conditions from 8mm to 40mm, and can be rated for fire high concern (SVHC) (17 January 2023) above a concentration
conditions. of 0.1% by mass: no."
Technical Data
2) "This product/article/at least one partial article contains other
The following structural properties are relevant for the declared CMR substances in categories 1A or 1B which are not on the
product EP 1000 as delivered: candidate list, exceeding 0.1 percentage by mass: no"
Construction Data
3) "Biocide products were added to this construction product or
Name Value Unit
it has been treated with biocide products (this then concerns a
Density acc. to DIN 51757 for mixing the two
1.4 g/cm³ treated product as defined by the (EU) Regulation on Biocidal
components
Products No. 528/2012): no"
Compressive strength acc. to DIN EN 196 Part 1 121.8N/mm²
Flexural strength acc. to DIN EN 196 Part 1 66 N/mm² The product considered in this EPD contains individual
components in the following ranges:
Storage:
Store in a cool, dry and dark place; storage temperature: +5°C
Resin component:
to +35°C
Epoxy resin: 40 to 75% by weight
Mineral fillers: 30 to 40% by weight
Shelf life:
Other components: < 5% by weight
24 months in cartridge systems
Curing agent component:
Gel and working time:
Various polyamines: 40 to 50% by weight
0°C 90 min.
Mineral fillers: 30 to 50% by weight
+ 5°C 80 min.
Other components: < 5% by weight
+ 10°C 60 min.
+ 15°C 40 min.
Reference service life
+ 20°C 30 min.
The declared product EP 1000 may be exposed to a wide
+ 25°C 12 min.
range of environmental conditions during the use phase. Its
+ 35°C 8 min.
expected reference service life depends on the specific
+ 40 °C 8 min.
installation situation and on the product's resulting exposure.
The main factors influencing service life are weather conditions
Curing time in dry substrate:
and mechanical and chemical stresses.
0°C 8640 min.
+ 5°C 2880 min.
LCA: Calculation rules
resin product in the ratio at which the two components must be
Declared Unit mixed before use. The mass mixing ratio between the resin
The product declared is a two-component reaction resin mortar component and the curing agent component is 4:1 (volume
manufactured by Chemofast Anchoring GmbH with the product ratio 3:1). The packaging is also included in the calculation at
name EP 1000. The declared unit is based on 1 kg reaction 0.1435 kg per 1 kg of reaction resin product. The declared unit
2 Environmental Product Declaration - Chemofast Anchoring GmbH - EP 1000
data are presented in the table below:
Declared unit data
Name Value Unit
Declared unit 1 kg
Other declared units are allowed if the conversion is shown
transparently.
System boundary
Type of EPD: Cradle to factory gate with options. The following
information modules are defined as system boundaries in this
study:
Production stage (A1–A3):
• A1, Raw material extraction,
• A2, Transport to the manufacturer,
• A3, Manufacturing. Figure 1 Information modules A1 to A3 of the product
End of life (C1-C4):
• C1, Deconstruction/demolition,
• C2, Transport,
• C3, Waste processing,
• C4, Disposal.
Reuse, recovery and recycling potential (D)
To precisely determine the indicators and environmental
Figure 2 Information modules A1 to A3 of the packaging
impacts of the declared unit, a total of 8 information modules
are considered. The information modules A1 to A3 describe the
Information modules C1 to C4 document
material provision, the transport to the production site, as well
deconstruction/demolition for removal from the building,
as the production processes of the product itself.
transport to waste disposal, waste processing and product
disposal. Reuse, recovery and recycling potential are
The precursor products are sourced from Germany. Transport
documented in information module D.
is exclusively done by truck. The following process diagrams
illustrate the underlying production process.
Geographic Representativeness
Land or region, in which the declared product system is
manufactured, used or handled at the end of the product´s
lifespan: Germany
Comparability
Basically, a comparison or an evaluation of EPD data is only
possible if all the data sets to be compared were created
according to EN 15804 and the building context, respectively
the product-specific characteristics of performance, are taken
into account.
The background datasets from the LCA for Experts and
ecoinvent 3.9.1 databases, which this study also draws on, are
documented at the following site (Sphera). 2023.1
http://www.gabi-software.com/deutsch/index/ (ecoinvent 3.9.1).
http://ecoquery.ecoinvent.org/3.9.1/cutoff/search
LCA: Scenarios and additional technical information
Name Value Unit
Characteristic product properties of biogenic carbon
Packaging PP 0.1188 kg
No renewable raw materials are used in the product or the
Packaging PA6 0.0082 kg
packaging. The biogenic carbon value is therefore reported as
zero. Packaging PE-LD 0.0165 kg
Packaging per declared unit End of Life (C1–C4)
The product is demolished by using an electric chisel. The
electrical energy consumption for this tool is estimated at 0.05
3 Environmental Product Declaration - Chemofast Anchoring GmbH - EP 1000
MJ for the declared unit. The power consumption is calculated
Reuse, recovery and recycling potential (D), relevant
using a European energy mix. Construcion waste is transported
scenario specifications
200 km by truck to a waste treatment facility. At the waste
The product has no reuse, recovery or recycling potential.
treatment facility, the construction waste is shredded and then
Information module D is therefore declared and reported as
disposed in a landfill.
zero.
Name Value Unit
Name Value Unit
Collected as mixed construction waste 1 kg
Reuse, recovery and recycling potential 0 kg
Shredding 1 kg
Disposal in landfill 1 kg
4 Environmental Product Declaration - Chemofast Anchoring GmbH - EP 1000
LCA: Results
The results in this calculation refer to the characterisation factors EN 15840+A2/EF 3.1.
DESCRIPTION OF THE SYSTEM BOUNDARY (X = INCLUDED IN LCA; MND = MODULE OR INDICATOR NOT DECLARED; MNR
= MODULE NOT RELEVANT)
Benefits and
Construction loads beyond
Product stage Use stage End of life stage
process stage the system
boundaries
la ire ta m w a Ry lp p u s tro p s n a rT g n iru tc a fu n a M e h t m o rf tro p s n a rTe tis e h t o t e ta g y lb m e s s A e s U e c n a n e tn ia M ria p e R tn e m e c a lp e R tn e m h s ib ru fe R y g re n e la n o ita re p Oe s u re ta w la n o ita re p Oe s u n o itc u rts n o c -e Dn o itilo m e d tro p s n a rT g n is s e c o rp e ts a W la s o p s iD -e s u e R-y re v o c e R-g n ilc y c e Rla itn e to p
A1 A2 A3 A4 A5 B1 B2 B3 B4 B5 B6 B7 C1 C2 C3 C4 D
X X X MND MND MND MND MNR MNR MNR MND MND X X X X X
RESULTS OF THE LCA - ENVIRONMENTAL IMPACT according to EN 15804+A2: 1 kg Chemofast EP 1000
Parameter Unit A1-A3 C1 C2 C3 C4 D
Global Warming Potential total (GWP-total) kg CO 2 eq 4.1E+00 4.58E-03 1.75E-02 2.58E-03 1.46E-02 0
Global Warming Potential fossil fuels (GWP-fossil) kg CO 2 eq 3.97E+00 4.53E-03 1.73E-02 2.56E-03 1.46E-02 0
Global Warming Potential biogenic (GWP-biogenic) kg CO 2 eq 1.26E-01 4.91E-05 0 0 0 0
Global Warming Potential luluc (GWP-luluc) kg CO 2 eq 8.91E-04 4.87E-07 1.58E-04 1.92E-05 4.53E-05 0
Depletion potential of the stratospheric ozone layer (ODP) kg CFC11 eq 2.19E-10 8.27E-14 1.49E-15 4.28E-15 3.71E-14 0
Acidification potential of land and water (AP) mol H+ eq 5.13E-03 9.57E-06 6.48E-05 1.34E-05 1.03E-04 0
Eutrophication potential aquatic freshwater (EP-freshwater) kg P eq 2.24E-05 1.67E-08 6.21E-08 8.71E-09 2.93E-08 0
Eutrophication potential aquatic marine (EP-marine) kg N eq 1.76E-03 2.29E-06 3.03E-05 6.13E-06 2.67E-05 0
Eutrophication potential terrestrial (EP-terrestrial) mol N eq 1.89E-02 2.39E-05 3.39E-04 6.77E-05 2.94E-04 0
Formation potential of tropospheric ozone photochemical oxidants kg NMVOC
5.94E-03 6.11E-06 5.84E-05 1.66E-05 8.06E-05 0
(POCP) eq
Abiotic depletion potential for non fossil resources (ADPE) kg Sb eq 2.08E-07 6.95E-10 1.1E-09 2.74E-09 6.72E-10 0
Abiotic depletion potential for fossil resources (ADPF) MJ 8.8E+01 9.43E-02 2.32E-01 5.04E-02 1.94E-01 0
m3 world eq
Water use (WDP) 1.21E-01 9.98E-04 1.96E-04 4.98E-04 1.6E-03 0
deprived
RESULTS OF THE LCA - INDICATORS TO DESCRIBE RESOURCE USE according to EN 15804+A2: 1 kg Chemofast EP 1000
Parameter Unit A1-A3 C1 C2 C3 C4 D
Renewable primary energy as energy carrier (PERE) MJ 8.76E+00 5.64E-02 1.64E-02 4.68E-03 3.16E-02 0
Renewable primary energy resources as material utilization
MJ 0 0 0 0 0 0
(PERM)
Total use of renewable primary energy resources (PERT) MJ 8.76E+00 5.64E-02 1.64E-02 4.68E-03 3.16E-02 0
Non renewable primary energy as energy carrier (PENRE) MJ 6.69E+01 9.43E-02 2.32E-01 5.05E-02 1.94E-01 0
Non renewable primary energy as material utilization (PENRM) MJ 2.11E+01 0 0 0 0 0
Total use of non renewable primary energy resources (PENRT) MJ 8.81E+01 9.43E-02 2.32E-01 5.05E-02 1.94E-01 0
Use of secondary material (SM) kg 0 0 0 0 0 0
Use of renewable secondary fuels (RSF) MJ 0 0 0 0 0 0
Use of non renewable secondary fuels (NRSF) MJ 0 0 0 0 0 0
Use of net fresh water (FW) m3 1.18E-02 4.55E-05 1.81E-05 1.44E-05 4.9E-05 0
RESULTS OF THE LCA – WASTE CATEGORIES AND OUTPUT FLOWS according to EN 15804+A2:
1 kg Chemofast EP 1000
Parameter Unit A1-A3 C1 C2 C3 C4 D
Hazardous waste disposed (HWD) kg 7.4E-09 7.38E-12 8.59E-13 1.31E-13 4.23E-12 0
Non hazardous waste disposed (NHWD) kg 6.94E-02 6.91E-05 3.35E-05 1.33E-05 9.71E-01 0
Radioactive waste disposed (RWD) kg 1.31E-03 1.5E-05 3E-07 6.77E-07 2.21E-06 0
Components for re-use (CRU) kg 0 0 0 0 0 0
Materials for recycling (MFR) kg 0 0 0 0 0 0
Materials for energy recovery (MER) kg 0 0 0 0 0 0
Exported electrical energy (EEE) MJ 0 0 0 0 0 0
Exported thermal energy (EET) MJ 0 0 0 0 0 0
RESULTS OF THE LCA – additional impact categories according to EN 15804+A2-optional:
1 kg Chemofast EP 1000
Parameter Unit A1-A3 C1 C2 C3 C4 D
Disease
Incidence of disease due to PM emissions (PM) ND ND ND ND ND ND
incidence
Human exposure efficiency relative to U235 (IR) kBq U235 eq ND ND ND ND ND ND
Comparative toxic unit for ecosystems (ETP-fw) CTUe ND ND ND ND ND ND
Comparative toxic unit for humans (carcinogenic) (HTP-c) CTUh ND ND ND ND ND ND
5 Environmental Product Declaration - Chemofast Anchoring GmbH - EP 1000
Comparative toxic unit for humans (noncarcinogenic) (HTP-nc) CTUh ND ND ND ND ND ND
Soil quality index (SQP) SQP ND ND ND ND ND ND
Disclaimer 2 - applies to the following indicators: 'Abiotic shortage potential - non-fossil resources', 'Abiotic shortage potential - fossil
fuels', 'Water deprivation potential (users)', 'Potential comparative toxic unit for ecosystems', 'Potential comparative toxic unit for human
health - carcinogenic effects', 'Potential comparative toxic unit for human health - non-carcinogenic effects', 'Potential soil quality index'.
The results of this environmental impact indicator shall be used with care, as the uncertainties of the results are high and as there is
limited experience with the indicator.
References
DIN 51757 ecoinvent 3.9.1
DIN 51757:2011-01 Testing of mineral oils and related Background database: ecoinvent 3.9.1 Ziirich: ecoinvent (Ed.)
materials - Determination of density. http://www.ecoinvent.org (26 May 2023)
EN 196 ETA-19/0201
DIN EN 196-1:2016-11 Methods of testing cement - Part 1: European Technical Assessment
Determination of strength.
ETA-19/0200
EN 15804 European Technical Assessment
EN 15804+A2:2019+AC:2021, Sustainability of construction
works - Environmental product declarations - Core rules for the IBU 2021
product category of construction products. Institut Bauen und Umwelt e.V.: General guidance for the EPD
programme of the Institut Bauen und Umwelt e.V., Version 2.0,
EN/TR 15941 Berlin: Institut Bauen und Umwelt e.V., 2021. www.ibu-epd.com
CEN/TR 15941:2010-03: Sustainability of construction works -
Environmental product declarations - Methodology for selection PCR Part A
and use of generic data Product Category Rules for Building-Related Products and
Services - Calculation Rules for Life Cycle Assessment and
ISO 14025 Requierements on the Project Report V1.3, Institut Bauen und
DIN EN ISO 14025:2011-10, Environmental labels and Umwelt e.V., 08.2022
declarations - Type III environmental declarations - Principles
and procedures. PCR: Reaction resin products
Guidance-Texts for Building-Related Products and Services-
ISO 14044 PART B: Requirements on the Environmental Product
DIN EN ISO 14044:2006-10, Environmental management - Life Declarations for Reaction Resin Products,1 August 2021
cycle assessment - Requirements and guidelines.
Sphera
Further references LCA for Experts: 2023.1 Leinfelden-Echterdingen; Sphera
Solution GmbH (Ed.) http://www. gabi-
ECHA candidates list software.com/deutsch/index/ (26 May 2023)
https://echa.europa.eu/de/candiate-list-substances-in-articles
Regulation (EU) No. 305/2011 (CPR)
ECHA list
https://echa.europa.eu/de/candiate-list-table Regulation (EU) No. 528/2012 (Biocidal Products Regulation)
6 Environmental Product Declaration - Chemofast Anchoring GmbH - EP 1000
Publisher
Institut Bauen und Umwelt e.V. +49 (0)30 3087748- 0
Hegelplatz 1 info@ibu-epd.com
10117 Berlin www.ibu-epd.com
Germany
Programme holder
Institut Bauen und Umwelt e.V. +49 (0)30 3087748- 0
Hegelplatz 1 info@ibu-epd.com
10117 Berlin www.ibu-epd.com
Germany
Author of the Life Cycle Assessment
FIT-Umwelttechnik GmbH 05362 72 69 474
Westerstr. 13 bertram@fit-umwelttechnik.de
38442 Wolfsburg www.fit-umwelttechnik.com
Germany
Owner of the Declaration
Chemofast Anchoring GmbH +49 2154 8123 0
Hanns-Martin-Schleyer-Str. 23 info@chemofast.de
47877 Willich www.chemofast.de
Germany
7 Environmental Product Declaration - Chemofast Anchoring GmbH - EP 1000
