ENVIRONMENTAL PRODUCT DECLARATION
as per ISO 14025 and EN 15804+A2
Owner of the Declaration Grundfos Holding A/S
Publisher Institut Bauen und Umwelt e.V. (IBU)
Programme holder Institut Bauen und Umwelt e.V. (IBU)
Declaration number EPD-GRU-20240016-CBA1-EN
Issue date 21.03.2024
Valid to 20.03.2029
MAGNA3 40-80/100 (Stainless Steel)
Grundfos Holding A/S
www.ibu-epd.com | https://epd-online.com
General Information
Grundfos Holding A/S MAGNA3 40-80/100 (Stainless Steel)
Programme holder Owner of the declaration
IBU – Institut Bauen und Umwelt e.V. Grundfos Holding A/S
Hegelplatz 1 Poul Due Jensens Vej 7
10117 Berlin 8850 Bjerringbro
Germany Denmark
Declaration number Declared product / declared unit
EPD-GRU-20240016-CBA1-EN 1 PCS. of MAGNA3 40-80/100 (Stainless Steel)
This declaration is based on the product category rules: Scope:
Pumps for liquids and liquids with solids, 01.08.2021 The declaration applies to 1 piece of MAGNA3 (Stainless Steel) pump. The
(PCR checked and approved by the SVR) product is produced in Wahlstedt, Germany, and the life cycle assessment
is based on data collected at the production site.
Issue date Production has been modeled using annual production data from 2021.
21.03.2024
The declaration covers two different types of the MAGNA3 40- product
(80/100).
The owner of the declaration shall be liable for the underlying information
Valid to
and evidence; the IBU shall not be liable with respect to manufacturer
20.03.2029 information, life cycle assessment data and evidences.
The EPD was created according to the specifications of EN 15804+A2. In
the following, the standard will be simplified as EN 15804.
Verification
The standard EN 15804 serves as the core PCR
Independent verification of the declaration and data according to ISO
14025:2011
internally X externally
Dipl.-Ing. Hans Peters
(Chairman of Institut Bauen und Umwelt e.V.)
Florian Pronold Mrs Kim Allbury,
(Managing Director Institut Bauen und Umwelt e.V.) (Independent verifier)
1 Environmental Product Declaration - Grundfos Holding A/S - MAGNA3 40-80/100 (Stainless Steel)
Product
Product description/Product definition Ecodesign Directive (2009/125/EC)
The Grundfos MAGNA3 circulator pumps are designed for
circulating liquids in heating systems, air conditioning and Commission Regulation (EC) No: 641/2009 and
cooling systems and domestic hot water systems. However, the
pump range can also be used in ground source heat pump Commission Regulation (EU) 622/2012
systems and solar heating systems.
Standards used:
The MAGNA3 pump is a centrifugal pump powered by an EN 16297-1:2012, EN 16297-2:2012, EN 16297-3:2012.
electrical motor. It has a high-performance neodymium magnet
rotor which increases motor efficiency and an insulation shell to The CE marking takes into account the proof of conformity with
reduce heat loss from the cast iron pump housing with threaded the respective harmonized norms based on the legal provisions
connections. above.
MAGNA3 pumps are not harmonized in accordance with the
The declaration covers two types of the MAGNA3 pump. They CPR.
are grouped as shown below. The group reference in the
technical data and scenarios refers also to these. GROUP 1 - Application
MAGNA3 40-80 For the application and use the respective nationalprovisions
apply.
GROUP 2 - MAGNA3 40-100
The pump is designed for circulating liquids in the
These are all the same physical products and 100 % identical
in terms of design, dimensions and materials as well as supply following systems:
chain and manufacturing processes, i.e., all cradle to gate
processes (A1-A3). · heating systems
The products are also identical in terms of packaging, · domestic hot-water systems
distribution, reference service life and end-of-life treatment.
· air-conditioning and cooling systems
The only thing that differentiates the products from each other
is the software which controls how the pump operates in the · ground-source heat-pump systems
system in which it is installed, making them fit for different
applications. Hence, all life cycle modules are identical, except · solar-heating systems
use stage module B6, which will change, as the applied
scenarios for electricity consumption changes. For the placing The pump is suitable for thin, clean, non-aggressive and non-
on the market in the European Union/European Free Trade explosive liquids, not containing solid particles or fibres that
Association (EU/EFTA) (with the exception of Switzerland) the may attack the pump mechanically or chemically. In heating
following legal provisions apply: systems, the water must meet the requirements of accepted
standards on water quality in heating systems. The pumps are
Machinery Directive (2006/42/EC) also suitable for domestic hot-water systems.
Standard used: EN 809:1998 + A1:2009. Technical Data
The performance data of the product according to the
Radio Equipment Directive (2014/53/EU) harmonized norms, based on the harmonization provisions
above apply.
Standards used:
EN 60335-1:2012/AC:2014 + A11:2014, EN 60335-2-51:2003 + The relevant technical specifications according to the PCR Part
A1:2008 + A2:2012, EN 62233:2008. B are given in the table below.
EN 55014-1:2006 + A1:2009 + A2:2011, EN 55014-1:2017, EN Characteristics that are the same for all product groups are only
61000-6-2:2005, EN 61000-3-2:2014, EN 61000-3-3:2013, given once. Others are given individually for all two groups.
ETSI EN 301 489-1 V2.2.0, ETSI EN 301 489-17 V3.2.0. ETSI Constructional data
EN 300 328 V2.1.1
Electromagnetic Compatibility (EMC) Directive
(2014/30/EU)
Standards used:
EN 55014-1:2017, EN 55014-2:2015,
EN 61000-3-2:2014/2019, EN 61000-6-2:2008/2019,
EN 61000-3-3:2013 A1:2019
RoHS Directive 2011/65/EU and 2015/863//EU
Standard: EN 50581:2012.
2 Environmental Product Declaration - Grundfos Holding A/S - MAGNA3 40-80/100 (Stainless Steel)
Name Value Unit REACH
This product/article/at least one partial article contains
Frequency 50 Hz
substances listed in the ECHA candidate list (date:
Voltage 230 V
Clean
Pumped liquid (e.g. water) - 10.06.2022) exceeding 0.1 percentage by mass: no
Water
Energy Efficiency Index Gr.1 0,19 The Wahlstedt production has been assessed and certified as
Energy Efficiency Index Gr.2 0,18 meeting the requirements in ISO 14001, ISO 50001, ISO 45001
Flow range Gr. 1 (max) 18,5 m3/h and ISO 9001.
Flow range Gr. 2 (max) 21,0 m3/h Reference service life
Head max. Gr.1 8 m No use stage scenario which refers to the lifetime of the product
Head max. Gr.2 10 m is declared. However, to facilitate building calculations, an
estimated RSL of 10 years can be used.
Power input Gr. 1 Average (from load profile
0,117 kW This is an EU consensus-based estimation, referenced on page
describing use)
37 in Appendix 7: Lot 11 – Circulators in Buildings, prepared by
Power input Gr. 2 Average (from load profile
0,163 kW AEA Energy & Environment for the European Commission in
describing use)
the context of the Eco Design Directive:
Nominal capacity Gr.1 0,267 kW
Nominal capacity Gr.2 0,359 kW There is no definitive information on the average circulator life
available, there is consensus within the industry that it is at
Performance data of the product according to the harmonised
least 12 years. However, this is complicated by many factors,
standards, based on provisions for harmonisation.
including many being scrapped prematurely when e.g. the
Base materials/Ancillary materials boiler they are connected to is replaced.
Base materials / Ancillary materials
From the estimated stock (140Mpa) and annual sales (14Mpa),
Name Value Unit the average lifetime of the circulator is taken as 10 years for the
Aluminium 16,15 % purposes of this study.
Ceramics 0,36 %
The RSL of the declared product is not directly influencing the
Copper 3,05 %
results in this study, as no declared use stage scenario is
Electronics 0,27 %
dependent on the RSL; The use stage sub-module B6 is
Magnet Nd 1,3 % declared per year as required by the PCR Part B.
Paper 0,6 %
PCB 4,47 %
Plastics 0,39 %
Plastics, foam 0,85 %
Plastics GF 6,17 %
Rubber 0,2 %
Stainless steel 51,68 %
Steel 6,08 %
Cardboard 8,33 %
Plastic film 0,08 %
TOTAL 100 %
LCA: Calculation rules
processes as well as the manufacturing process. The final
Declared Unit production and assembly of the MAGNA3 pump takes place at
The declared unit is 1 piece (pcs.) of MAGNA3 (Stainless Steel) a Grundfos manufacturing site in Germany. However, the full
pump. supply-chain leading to the finished product at the gate is rather
Declared unit complex and includes a large amount of raw materials,
components and semi-finished parts which comes from both
Name Value Unit
external suppliers as well as other Grundfos production facilities
Declared unit 1 pce.
Mass reference 19.22 kg/pce The product stage is included in the study, and according to EN
Conversion factor [Mass/Declared Unit] 19.22 15804 the system boundary with nature is set to include those
System boundary processes that provide the material and energy inputs into the
system and the following manufacturing, transport up to the
This EPD is Cradle-To-Grave. The system boundaries
factory gate as well as the processing any waste arising from
those processes.
of the EPD follow the modular approach in EN 15804.
By decision no. 20170712-n of the SVR, the modules B3, B4
Wastes and losses are included in the modules where they
and B5 are by default declared as "MNR" (module not relevant).
occur according to the polluter pays principle and the modular
approach of EN 15804.
The product stage (A1-A3)
comprises raw material extraction and processing, transport
The product includes:
3 Environmental Product Declaration - Grundfos Holding A/S - MAGNA3 40-80/100 (Stainless Steel)
The packaging material does not reach the end of waste state
· A1 Extraction and processing of raw materials; but is incinerated as waste. According to European statistics,
the average R1 value of incineration plants is > 0.6. Therefore,
· A1 Reuse of products or materials from a previous product it is assumed
system;
that packaging material is treated thermally in an incineration
· A1 Processing of secondary materials; plant with R1 > 0.6. The loads from the combustion process of
packaging are declared in module A5 and the resulting energy
· A1 Generation of electricity, steam and heat from primary benefits in module
energy resources, also including their extraction, refining and
transport; D, as required by the PCR Part A, 5.5.2.
· A1 Energy recovery and other recovery processes from Use stage (B1-B7):
secondary fuels;
The use stage, related to the building fabric includes:
· A2 Transportation up to the factory gate and internal transport;
· B1, use or application of the installed product;
· A3 Production of ancillary materials or pre products;
· B2, maintenance.
· A3 Manufacturing of products and coproducts;
The use stage related to the operation of the building
· A3 Manufacturing of packaging;
includes:
· A1-A3 processing up to the end-of-waste state or disposal of
final residues. · B6, operational energy use;
For secondary material inputs, the system boundary to the · B7, operational water use.
previous system (providing the secondary material) is set where
outputs reach the end-of-waste state. The recycling of In this study, all use stage modules are assessed, though B1,
secondary material into new raw materials is included in the B2 and B7 are assessed to be zero. By decision no. 20170712-
system boundary of this study. Waste n of the SVR, the modules B3, B4 and B5 are by default
declared as "MNR" (module
materials from production processes that are recycled without
any modification of the material's inherent characteristics are not relevant). The modules include the provision and transport
modelled as closed-loop within A1-A3. This is done up to the of all materials, products and related energy and water use, as
input mass flow that was used during production. well as waste processing up to the end-of-waste state or
disposal of final residues during the use stage. They also
Waste for incineration arising in the product stage is accounted include all impacts and
for in the module where the waste is produced. The
environmental loads from the incineration process are declared aspects related to the losses during the use stage (i.e.
in the module where it occurs and the electricity and heat which production, transport, and waste processing and disposal of the
are produced from the incineration is considered as closed-loop lost products and materials).
within A1-A3, as described in PCR Part A,
5.5.1. The input of biogenic carbon from the production of Generally, the geographical coverage of the datasets used
packaging material is inventoried in A3. As required by PCR matches the actual processes taking place. Meaning, that when
Part A, the corresponding end-of-life module of the packaging modelling taking place in Grundfos Bjerringbro, the Danish
material, A5, is also declared and the emissions of biogenic electricity grid mix is used in the model and thermal energy
carbon are inventoried. from natural gas. These are generally of very high quality with
very good technological, temporal and geographical
The construction process stage (A4-A5) includes: representativeness.
A4: Contributions to operational energy use during the use stage
(B6) come from the electricity consumption of the product. The
· Transportation from factory gate to the distribution center: annual electricity consumption is calculated by multiplying the
average power input, which is based on a defined load profile,
· Consumption of electricity, thermal energy and water at the with the annual running hours. For use stage (B6) European
distribution center; Average electricity grid mix has been used. These values are
declared in the scenarios section.
· Transportation from distribution center to construction site;
The End-of-Life stage (C1-C4)
· Wastage during distribution. includes all activities from when the product reaches the end of
its service life and no longer provides any functionality and until
A5: all materials and components are processed for
· Installation process; reuse/recycling or disposed of.
· Transport of packaging waste to treatment site; According to EN 15804 and the PCR Part A,
the end-of-life stage includes:
· Waste treatment of packaging.
· C1 deconstruction of the product from the
4 Environmental Product Declaration - Grundfos Holding A/S - MAGNA3 40-80/100 (Stainless Steel)
Beyond system boundary (D):
· building, including initial on-site sorting of the According to EN 15804 module D includes the reuse, recovery
and/or recycling potentials, expressed as net impacts and
· materials; benefits. Any declared benefits and loads from net
· C2 transportation of the discarded product to a recycling site flows leaving the product system that have not been allocated
and transportation of waste to final disposal; as co-products and that have passed the end-of-waste state
are included in module D.
· C3 waste processing, collection of waste fractions from the
deconstruction and waste processing of material flows intended Contributions to module D comes from waste incineration
for reuse, recycling and energy recovery; processes in A5 and C3 as well as material recycling in C3. The
specific fractions and net flows are shown in the scenarios
· C4 waste disposal including physical pretreatment and section.
management of the disposal site.
Comparability
At the end of life, the MAGNA3 pump is manually disassembled
from the piping system in which it has been installed. The Basically, a comparison or an evaluation of EPD data is only
definition of the applied end-of-life scenario in this EPD follows possible if all the data sets to be compared were created
the requirements in the according to EN 15804 and the building context, respectively
the product-specific characteristics of performance, are taken
PCR Part A, 6.2 regarding complex products, with a into account.
combination of recycling, thermal waste treatment and
landfilling. 100 % of the material is considered in the end of life
scenario as required by the PCR. Geographic Representativeness
An overall collection rate of 90 % has been assumed. Land or region, in which the declared product system is
manufactured, used or handled at the end of the product´s
Materials from which energy is recovered in an incineration lifespan: Europe
process with an R1-value above 0.60 are in this study included
with the environmental burdens from the incineration process
Comparability
inventoried in C3, the recovered energy is declared as exported
Basically, a comparison or an evaluation of EPD data is only
energy in C3
possible if all the data sets to be compared were created
according to EN 15804 and the building context, respectively
and the energy benefits are declared in D. This procedure is
the product-specific characteristics of performance, are taken
according to the PCR Part A, 5.5.6. C3 includes the mechanical
into account. Software and databases used: LCA for Experts
separation of the product followed by a series of sorting steps.
10.7.1.28
Metal fractions are recycled and plastics, cardboard and
Schema 8007
electronics are assumed incinerated with energy recovery. The
Sphera and Ecoinvent databases
residual fractions are landfilled and declared in C4.
The specific amounts are shown in the scenarios section.
LCA: Scenarios and additional technical information
Name Value Unit
Characteristic product properties of biogenic carbon
Litres of fuel 0,0332 l/100km
The biogenic carbon content quantifies the amount of biogenic
Transport distance 2003 km
carbon in a construction product leaving the factory gate, and it
will be separately declared for the product and for any Capacity utilisation (including empty runs) 85 %
accompanying packaging, as required from the PCR Part A. Gross density of products transported 360 kg/m3
The Carbon content of Cardboard and Paper is assumed to
Wastage during distribution 0,02 %
0.46 kg C generally. This means that 46% of the weight of
paper and cardboard is assumed to be biogenic carbon. Installation into the building (A5)
Overall, there is an amount of weight-% Carbon in the product
Name ValueUnit
leaving the factory gate and it has to be considered.
Packaging waste for incineration (LDPE film) 0,016 kg
Packaging waste for incineration
Information on describing the biogenic Carbon Content at 1,717 kg
(Paper/Cardboard)
factory gate
An estimated
Name ValueUnit
RSL of 10 years can be used to facilitate building calculations.
Biogenic carbon content in accompanying kg
0.79 This is an EU
packaging C
consensus-based estimation, referenced in Appendix 7: Lot 11
Note: 1 kg of biogenic carbon is equivalent to 44/12 kg of CO2 – Circulators in
Buildings, prepared by AEA Energy & Environment for the
European Commission
in the context of the Eco Design Directive.
Transport from the gate to the site (A4) Reference service life
Name Value Unit
Life Span according to the manufacturer 10 a
5 Environmental Product Declaration - Grundfos Holding A/S - MAGNA3 40-80/100 (Stainless Steel)
Operational energy use (B6) Reuse, recovery and/or recycling potentials (D), relevant
Name Value Unit scenario information
Electricity consumption, Group 1 585 kWh/a Name Value Unit
Electricity consumption, Group 2 815 kWh/a A5, incineration w/energy recov. thermal energy 7,97 MJ
Average power input, Group 1 0,117 kW A5, incineration w/energy recov. electric energy 4,41 MJ
Average power input, Group 2 0,163 kW C3, steel for recycling (net amounts) -0,333 kg
Running hours (all groups) 5.000 h/a C3, stainless steel for recycling (net amounts) 2,67 kg
C3, aluminium for recycling (net amounts) -0,434 kg
End of life (C1-C4)
C3, copper for recycling (net amounts) 0,221 kg
Name Value Unit
C3, incineration w/energy recov. thermal energy. 12,6 MJ
Collected as mixed construction waste 17,488 kg
C3, incineration w/energy recov. electric energy 6,97 MJ
Transportation distance (C2) 500 km
Aluminium for recycling 2,74 kg
Steel for recycling 1,03 kg
Copper for recycling 0,52 kg
Stainless steel for recycling 8,76 kg
Plastics for incineration w/energy 1,29 kg
Electronics for incineration w/energy 0,80 kg
Landfilling 2,34 kg
6 Environmental Product Declaration - Grundfos Holding A/S - MAGNA3 40-80/100 (Stainless Steel)
LCA: Results
Characterization model: EN 15804 - 2012+A2 - 2019, PEF. By Decision no. 20170712-n of the IBU SVR, the modules B3, B4, B5 are
marked as MNR (module not relevant) as default. The LCA results in module B6 are given on a period of one year, according to PCR
Part B. To obtain the results from module B6 over the entire life cycle, the LCA results of module B6 must be multiplied by the
estimated RSL of 10 years. The indicator results for module B6 are declared for Group 1. B6 indicator results for other groups can be
derived by multiplying the B6 indicator results with the following factors:
Group 2: 1,39
DESCRIPTION OF THE SYSTEM BOUNDARY (X = INCLUDED IN LCA; MND = MODULE OR INDICATOR NOT DECLARED; MNR
= MODULE NOT RELEVANT)
Benefits and
Construction loads beyond
Product stage Use stage End of life stage
process stage the system
boundaries
la ire ta m w a Ry lp p u s tro p s n a rT g n iru tc a fu n a M e h t m o rf tro p s n a rTe tis e h t o t e ta g y lb m e s s A e s U e c n a n e tn ia M ria p e R tn e m e c a lp e R tn e m h s ib ru fe R y g re n e la n o ita re p Oe s u re ta w la n o ita re p Oe s u n o itc u rts n o c -e Dn o itilo m e d tro p s n a rT g n is s e c o rp e ts a W la s o p s iD -e s u e R-y re v o c e R-g n ilc y c e Rla itn e to p
A1 A2 A3 A4 A5 B1 B2 B3 B4 B5 B6 B7 C1 C2 C3 C4 D
X X X X X X X MNR MNR MNR X X X X X X X
RESULTS OF THE LCA - ENVIRONMENTAL IMPACT according to EN 15804+A2: 1PCS of MAGNA3 40-80/100
Parameter Unit A1 A2 A3 A4 A5 B1 B2 B6 B7 C1 C2 C3 C4 D
GWP-total kg CO 2 eq 9.85E+01 4.16E+00 8.22E-01 1.47E+00 2.83E+00 0 0 1.9E+02 0 0 6.01E-01 5.58E+00 1.16E-01 -7.94E+00
GWP-fossil kg CO 2 eq 9.84E+01 4.16E+00 3.62E+00 1.48E+00 4.61E-01 0 0 1.89E+02 0 0 6.04E-01 5.56E+00 1.17E-01 -7.92E+00
GWP- -2.83E
biogenic kg CO 2 eq -3.75E-03 -7.35E-03 +00 -2.18E-02 2.37E+00 0 0 1.64E+00 0 0 -8.92E-03 1.22E-02 -1.45E-03 -2.11E-02
GWP-luluc kg CO 2 eq 6.06E-02 6.71E-03 2.95E-02 1.34E-02 8.54E-05 0 0 2.05E-02 0 0 5.6E-03 1.82E-04 1.06E-04 -2.44E-03
kg CFC11
ODP 4.73E-08 3.29E-13 4.06E-09 2E-11 3.77E-13 0 0 3.48E-09 0 0 7.87E-14 2.65E-11 1.96E-13 -2.16E-11
eq
AP mol H+ eq 7.28E-01 1.23E-01 1.63E-02 8.81E-03 7.62E-04 0 0 4.03E-01 0 0 3.64E-03 3.77E-03 3.62E-04 -7.46E-02
EP-
kg P eq 1.49E-03 3.41E-06 6.21E-05 5.65E-06 1.4E-07 0 0 7.04E-04 0 0 2.21E-06 7.5E-06 1.35E-05 -1.14E-05
freshwater
EP-marine kg N eq 7.93E-02 2.93E-02 3.64E-03 4.25E-03 2.78E-04 0 0 9.64E-02 0 0 1.77E-03 9.95E-04 8.62E-05 -8.56E-03
EP-terrestrial mol N eq 8.48E-01 3.21E-01 3.65E-02 4.71E-02 3.5E-03 0 0 1.01E+00 0 0 1.96E-02 1.13E-02 9.47E-04 -9.19E-02
kg
POCP NMVOC 2.49E-01 8.27E-02 1.02E-02 8.09E-03 7.24E-04 0 0 2.57E-01 0 0 3.36E-03 2.66E-03 2.72E-04 -2.76E-02
eq
ADPE kg Sb eq 8.32E-03 7.91E-08 5.16E-05 1.25E-06 3.87E-09 0 0 2.92E-05 0 0 4.01E-08 2.21E-07 3.15E-09 -1.02E-03
ADPF MJ 1.39E+03 5.19E+01 5.39E+01 2.02E+01 1.04E+00 0 0 3.97E+03 0 0 8.24E+00 3.09E+01 1.75E+00 -9.48E+01
m3 world
WDP eq 3.48E+01 1.44E-02 3.97E-03 2.38E-02 3.39E-01 0 0 4.21E+01 0 0 7.31E-03 7.44E-01 -1.63E-03 -5.33E-01
deprived
GWP = Global warming potential; ODP = Depletion potential of the stratospheric ozone layer; AP = Acidification potential of land and water; EP =
Eutrophication potential; POCP = Formation potential of tropospheric ozone photochemical oxidants; ADPE = Abiotic depletion potential for non-fossil
resources; ADPF = Abiotic depletion potential for fossil resources; WDP = Water (user) deprivation potential)
RESULTS OF THE LCA - INDICATORS TO DESCRIBE RESOURCE USE according to EN 15804+A2: 1PCS of MAGNA3 40-
80/100
Parameter Unit A1 A2 A3 A4 A5 B1 B2 B6 B7 C1 C2 C3 C4 D
PERE MJ 3.74E+02 8.96E-01 4.99E+01 1.57E+00 2.35E-01 0 0 2.37E+03 0 0 6E-01 1.8E+01 1.58E-01 4.67E+00
-9.47E
PERM MJ 0 0 0 0 0 0 0 3.97E+03 0 0 8.27E+00 3.09E+01 1.75E+00
+01
PERT MJ 3.74E+02 8.96E-01 4.99E+01 1.57E+00 2.35E-01 0 0 2.37E+03 0 0 6E-01 1.8E+01 1.58E-01 4.67E+00
-9.47E
PENRE MJ 1.39E+03 5.2E+01 5.39E+01 2.03E+01 1.04E+00 0 0 3.97E+03 0 0 8.27E+00 3.09E+01 1.75E+00
+01
PENRM MJ 0 0 0 0 0 0 0 0 0 0 0 0 0 0
PENRT MJ 1.39E+03 5.2E+01 5.39E+01 2.03E+01 1.04E+00 0 0 0 0 0 0 0 0 0
SM kg 1.11E+01 0 2.31E-01 2.81E-03 0 0 0 0 0 0 0 0 0 0
RSF MJ 1.46E-23 0 0 2.99E-27 0 0 0 1.92E+00 0 0 6.57E-04 2.44E-02 1.83E-05 2.58E-02
NRSF MJ 1.71E-22 0 0 3.51E-26 0 0 0 2.37E+03 0 0 6E-01 1.8E+01 1.58E-01 4.67E+00
FW m3 1.03E+00 1.02E-03 1.99E-02 1.77E-03 8E-03 0 0 2.37E+03 0 0 6E-01 1.8E+01 1.58E-01 4.67E+00
PERE = Use of renewable primary energy excluding renewable primary energy resources used as raw materials; PERM = Use of renewable primary
energy resources used as raw materials; PERT = Total use of renewable primary energy resources; PENRE = Use of non-renewable primary energy
excluding non-renewable primary energy resources used as raw materials; PENRM = Use of non-renewable primary energy resources used as raw
7 Environmental Product Declaration - Grundfos Holding A/S - MAGNA3 40-80/100 (Stainless Steel)
materials; PENRT = Total use of non-renewable primary energy resources; SM = Use of secondary material; RSF = Use of renewable secondary fuels;
NRSF = Use of non-renewable secondary fuels; FW = Use of net fresh water
RESULTS OF THE LCA – WASTE CATEGORIES AND OUTPUT FLOWS according to EN 15804+A2:
1PCS of MAGNA3 40-80/100
Parameter Unit A1 A2 A3 A4 A5 B1 B2 B6 B7 C1 C2 C3 C4 D
HWD kg 7.01E-06 1.63E-10 1.21E-04 7.1E-08 2.6E-11 0 0 4.67E-07 0 0 2.56E-11 3.49E-09 1.46E-10 -1.66E-03
NHWD kg 7.41E+00 5.35E-03 3.53E-01 4.08E-03 1.13E-01 0 0 2.91E+00 0 0 1.26E-03 5.56E-01 2.03E+00 1.84E+00
RWD kg 4.74E-02 6.79E-05 1.66E-03 5.22E-05 4.72E-05 0 0 6.31E-01 0 0 1.55E-05 4.77E-03 2.06E-05 -1.8E-03
CRU kg ND ND ND ND ND ND ND ND ND ND ND ND ND ND
MFR kg 0 0 0 0 0 0 0 0 0 0 0 1.3E+01 0 0
MER kg ND ND ND ND ND ND ND ND ND ND ND ND ND ND
EEE MJ 0 0 0 0 4.41E+00 0 0 0 0 0 0 6.97E+00 0 0
EET MJ 0 0 0 0 7.97E+00 0 0 0 0 0 0 1.26E+01 0 0
HWD = Hazardous waste disposed; NHWD = Non-hazardous waste disposed; RWD = Radioactive waste disposed; CRU = Components for re-use;
MFR = Materials for recycling; MER = Materials for energy recovery; EEE = Exported electrical energy; EET = Exported thermal energy
RESULTS OF THE LCA – additional impact categories according to EN 15804+A2-optional:
1PCS of MAGNA3 40-80/100
Parameter Unit A1 A2 A3 A4 A5 B1 B2 B6 B7 C1 C2 C3 C4 D
Disease
PM 8.94E-06 2.12E-06 2.55E-07 5.65E-08 4.54E-09 0 0 3.39E-06 0 0 2.3E-08 3.2E-08 3.67E-09 -1.83E-06
incidence
kBq U235
IR 6.22E+00 9.83E-03 2.68E-01 7.43E-03 7.36E-03 0 0 1.05E+02 0 0 2.31E-03 7.94E-01 3.05E-03 -1.23E-01
eq
ETP-fw CTUe 7.23E+02 3.67E+01 1.88E+01 1.43E+01 5.06E-01 0 0 1.1E+03 0 0 5.91E+00 8.96E+00 1.1E+00 -1.15E+01
HTP-c CTUh 1.64E-05 6.84E-10 6.46E-07 7.64E-10 2.76E-11 0 0 5.84E-08 0 0 1.2E-10 5.03E-10 7.06E-11 -3.65E-07
HTP-nc CTUh 1.54E-06 2.36E-08 3.81E-08 1.32E-08 1.06E-09 0 0 9.32E-07 0 0 5.34E-09 1.04E-08 6.03E-09 -4.31E-08
SQP SQP 3.43E+02 4.22E+00 9.34E+01 8.35E+00 3.05E-01 0 0 1.56E+03 0 0 3.44E+00 1.2E+01 1.57E-01 -1.61E+01
PM = Potential incidence of disease due to PM emissions; IR = Potential Human exposure efficiency relative to U235; ETP-fw = Potential comparative
Toxic Unit for ecosystems; HTP-c = Potential comparative Toxic Unit for humans (cancerogenic); HTP-nc = Potential comparative Toxic Unit for humans
(not cancerogenic); SQP = Potential soil quality index
Disclaimer 1 – for the indicator 'Potential Human exposure efficiency relative to U235'.
This impact category deals mainly with the eventual impact of low-dose ionizing radiation on human health of the nuclear fuel cycle. It
does not consider effects due to possible nuclear accidents, occupational exposure or radioactive waste disposal in underground
facilities. Potential ionizing radiation from the soil, radon and from some construction materials is also not measured by this indicator.
Disclaimer 2 – for the indicators 'abiotic depletion potential for non-fossil resources', 'abiotic depletion potential for fossil resources',
'water (user) deprivation potential, deprivation-weighted water consumption', 'potential comparative toxic unit for ecosystems', 'potential
comparative toxic unit for humans – cancerogenic', 'Potential comparative toxic unit for humans - not cancerogenic', 'potential soil
quality index'. The results of this environmental impact indicator shall be used with care as the uncertainties on these results are high
as there is limited experience with the indicator.
Disclaimer 3: JRC Technical Reports, Version 2, 2018 Page 6, for the indicator "EP-freshwater". This indicator has been calculated as
'kg P eq' as required in the characterization model EUTREND model, Struijs et al., 2009b, as implemented in ReCiPe; This EPD was
created using a software tool.
References
Standards
PARLIAMENT AND OF THE COUNCIL of 26 February
Machinery Directive
2014 on the harmonistion of the laws of the Member
DIRECTIVE 2006/42/EC OF THE EUROPEAN
States relating to electromagnetic compatibility
PARLIAMENT AND OF THE COUNCIL of 17 May
Ecodesign Directive
2006 on machinery
DIRECTIVE 2009/125/EC OF THE EUROPEAN
Radio Equipment Directive
PARLIAMENT AND OF THE COUNCIL of 21 October
DIRECTIVE 2014/53/EU OF THE EUROPEAN PARLIAMENT
AND OF THE COUNCIL of 16 April 2014 on the harmonisation 2009 establishing a framework for the setting of
of the laws of the Member States relating to the making
available on the market of ecodesign requirements for energy-related products
radio equipment EC 641/2009
Electromagnetic Compatibility (EMC) Directive COMMISSION REGULATION (EC) No 641/2009 of 22 July
2009 implementing Directive 2005/32/EC of the European
DIRECTIVE 2014/30/EU OF THE EUROPEAN Parliament and of the Council with regard to ecodesign
8 Environmental Product Declaration - Grundfos Holding A/S - MAGNA3 40-80/100 (Stainless Steel)
requirements for glandless standalone circulators and family standard (CISPR 14-2:2015)
glandless circulators integrated in
EN 50581:2012
products
EN 50581:2012, Technical documentation for the
EC 622/2012
assessment of electrical and electronic products with
COMMISSION REGULATION (EU) No 622/2012 of 11 July
2012 amending Regulation (EC) No 641/2009 with regard to respect to the restriction of hazardous substances
ecodesign requirements for glandless standalone circulators
and glandless circulators integrated in products EN 60335-1
DIRECTIVE 2011/65/EU EN 60335-1:2012/A11:2014/A13:2017, Household
DIRECTIVE 2011/65/EU OF THE EUROPEAN and similar electrical appliances – Safety – Part 1:General
requirements
PARLIAMENT AND OF THE COUNCIL of 8 June 2011
EN 60335-2-51
on the restriction of the use of certain hazardous
EN 60335-2-51:2003-03 + A1:2008 + A2:2012, Household and
substances in electrical and electronic equipment similar electrical appliances – Safety –Part 2-51: Particular
requirements for stationary circulation pumps for heating and
DIRECTIVE 2015/863/EU service water installations
DIRECTIVE 2015/863/EU of 31 March 2015 amending EN 61000-3-2
Annex II to Directive 2011/65/EU of the European EN 61000-3-2:2014/2019, Electromagnetic compatibility (EMC)
– Part 3-2: Limits – Limits for harmonic current emissions
Parliament and of the Council as regards the list of (equipment input current =16 A per phase)
restricted substances EN 61000-3-3
ETSI EN 301 489-1 EN 61000-3-3:2013-08/ A1:2019, Electromagnetic compatibility
(EMC) – Part 3-3:
ETSI EN 301 489-1 V2.2.0, Electromagnetic Compatibility Limits – Limitation of voltage changes, voltage fluctuations and
(EMC) standard for radio equipment and services; Part 1: flicker in public low voltage supply systems, for equipment with
Common technical requirements
rated current <= 16 A per phase and not subject to conditional
ETSI EN 301 489-17 connection
ETSI EN 301 489-17 V3.2.0, Electromagnetic Compatibility EN 61000-6-2
(EMC) standard for radio equipment and services; Part 17:
Specific conditions for Broadband Data Transmission Systems EN 61000-6-2:2008/2019, Electromagnetic compatibility (EMC)
– Part 6-2: Generic standards –Immunity for industrial
ETSI EN 300 328 V2.1.1 environments
ETSI EN 300 328 V2.1.1, Wideband transmission systems; EN 16297-1
Data transmission equipment operating in the 2,4 GHz ISM
band and using wide band modulation techniques EN 16297-1:2012-10, Pumps – Rotodynamic pumps –
Glandless circulators – Part 1:
EN 809 General requirements and procedures for testing and
calculation of energy efficiency index (EEI)
EN 809:1998-10 + A1:2009, Pumps and pump units for
EN 16297-2
liquids - Common safety requirements
EN 16297-2:2012-10, Pumps – Rotodynamic pumps –
EN 55014-1 Glandless circulators – Part 2: Calculation of energy efficiency
index (EEI) for standalone circulators
EN 55014-1:2017, Electromagnetic compatibility –
Requirements for household appliances, electric tools and EN 16297-3
similar apparatus – Part 1: Emission
EN 16297-3:2012, Pumps – Rotodynamic pumps –Glandless
EN 55014-2 circulators – Part 3: Energy efficiency index (EEI) for circulators
integrated in products
EN 55014-2:2015, Electromagnetic compatibility –
ISO 14001
Requirements for household appliances, electric tools
EN ISO 14001:2015-09, Environmental management systems -
and similar apparatus – Part 2: Immunity – Product Requirements with guidance for use
9 Environmental Product Declaration - Grundfos Holding A/S - MAGNA3 40-80/100 (Stainless Steel)
ISO 14025 CML 2001
DIN EN /ISO 14025:2011-10, Environmental labels and Impact assessment characterization factors Institute of
declarations — Type III environmental declarations — Environmental Sciences, Leiden University, Netherlands
Principles and procedures
ECHA candidate list
EN 15804
Candidate List of substances of very high concern (SVHCs) for
EN 15804:2012-04+A1 2013, Sustainability of construction authorisation, European Chemicals Agency (ECHA), Helsinki,
works — Environmental Product Declarations — Core rules for Finland
the product category of construction products
EUTREND model
PCR Part A
Struijs et al., 2009b
Institut Bauen und Umwelt e.V., Berlin (pub.): Product Category AEA Energy & Environment
Rules for Building-Related Products and Services, Product
Category Rules for Construction Products from the range of
Environmental Product Declarations of Institut Bauen und Circulators in Buildings
Umwelt (IBU), Part A: Calculation Rules for the Life Cycle
Assessment and Requirements on the Project Report, Version Ecoinvent
1.7 (2021) Ecoinvent v3.9.1
PCR Part B LCA for ExpertsLCA for Experts
Institut Bauen und Umwelt e.V., Berlin (pub.): Product Category 10.7.1.28Schema 8007
Rules for Building-Related Products and Services, Product
Category Rules for Construction Products from the range of REACH
Environmental Product Declarations of Institut Bauen und
Umwelt (IBU), Part B: Requirements on the EPD for Pumps for Regulation (EC) No 1907/2006 of the European Parliament and
liquids and liquids with solids, Version 1.0 (2018) of the Council of 18 December 2006 concerning the
Registration, Evaluation, Authorisation and Restriction of
Further references Chemicals (REACH) (Status: 27.06.2018)
CPR SVR
REGULATION (EU) No 305/2011 OF THE EUROPEAN Advisory Board (formerly SVA)
PARLIAMENT AND OF THE COUNCIL of 9 March 2011 laying
down harmonised conditions for the marketing of construction Decision no.
products and repealing Council Directive 89/106/EEC 20170712-n
10 Environmental Product Declaration - Grundfos Holding A/S - MAGNA3 40-80/100 (Stainless Steel)
Publisher
Institut Bauen und Umwelt e.V. +49 (0)30 3087748- 0
Hegelplatz 1 info@ibu-epd.com
10117 Berlin www.ibu-epd.com
Germany
Programme holder
Institut Bauen und Umwelt e.V. +49 (0)30 3087748- 0
Hegelplatz 1 info@ibu-epd.com
10117 Berlin www.ibu-epd.com
Germany
Author of the Life Cycle Assessment
Grundfos Holding A/S +4587501400
Poul Due Jensens Vej 7 LCA_EPD@grundfos.com
8850 Bjerringbro www.grundfos.com
Denmark
Owner of the Declaration
Grundfos Holding A/S +4587501400
Poul Due Jensens Vej 7 LCA_EPD@grundfos.com
8850 Bjerringbro www.grundfos.com
Denmark
11 Environmental Product Declaration - Grundfos Holding A/S - MAGNA3 40-80/100 (Stainless Steel)
