ENVIRONMENTAL PRODUCT DECLARATION
as per ISO 14025 and EN 15804+A2
Owner of the Declaration dormakaba International Holding GmbH
Publisher Institut Bauen und Umwelt e.V. (IBU)
Programme holder Institut Bauen und Umwelt e.V. (IBU)
Declaration number EPD-DOR-20220159-CBA1-EN
Issue date 20.10.2022
Valid to 19.10.2027
Rack and pinion door closer TS Match and TS Match X
dormakaba
www.ibu-epd.com | https://epd-online.com
General Information
dormakaba Rack and pinion door closer TS Match and TS
Match X
Programme holder Owner of the declaration
IBU – Institut Bauen und Umwelt e.V. dormakaba International Holding GmbH
Hegelplatz 1 DORMA Platz 1
10117 Berlin 58256 Ennepetal
Germany Germany
Declaration number Declared product / declared unit
EPD-DOR-20220159-CBA1-EN 1 door closer (1 piece) of the TS Match
This declaration is based on the product category rules: Scope:
Building Hardware products, 01.08.2021 This Environment Product Declaration refers to a specific door closer
(PCR checked and approved by the SVR) manufactured by dormakaba Production GmbH & Co. KG. The production
site is located in Singapore.
Issue date The data represents the year 2020.
The owner of the declaration shall be liable for the underlying information
20.10.2022
and evidence; the IBU shall not be liable with respect to manufacturer
information, life cycle assessment data and evidences.
Valid to
The EPD was created according to the specifications of EN 15804+A2. In
19.10.2027 the following, the standard will be simplified as EN 15804.
Verification
The standard EN 15804 serves as the core PCR
Independent verification of the declaration and data according to ISO
14025:2011
internally X externally
Dipl.-Ing. Hans Peters
(Chairman of Institut Bauen und Umwelt e.V.)
Florian Pronold Dr.-Ing. Wolfram Trinius,
(Managing Director Institut Bauen und Umwelt e.V.) (Independent verifier)
1 Environmental Product Declaration - dormakaba - Rack and pinion door closer TS Match and TS Match X
Product
Product description/Product definition Base materials/Ancillary materials
The TS Match and TS Match X supplements the The major material composition including the packaging of the
comprehensive slide channel door closer range from product is listed below:
dormakaba. The closing speed is infinitely adjustable and with Name Value Unit
the concealed mounting plate which is optionally available, the
Aluminium 42 %
TS Match is the perfect door closers for the initial equipment of
Steel 39 %
the door. For the use and application of the product the
respective national provisions at the place of use apply. The Paper 11 %
standards which can be applied are the following: Lubricants 6 %
• EN 1154 Plastics 1 %
Zinc 1 %
Application
Others <1 %
The door closer series is designed for commercial and
institutional applications and is suitable for internal and external The products include partial articles which contain substances
doors. It can be used in a variety of applications, including as listed in the Candidate List of REACH
door closer for fire, anti-flame and smoke check doors (non- Regulation 1907/2006/EC (date: 17.02.2022) exceeding 0.1
hold-open versions). percentage by mass: yes
• Lead (Pb): 7439-92-1 (CAS-No.) is included in some of
Technical Data
the alloys used. The concentration of lead in each
The door closer series has following technical properties:
individual alloy does not exceed 4.0% (by mass).
The Candidate List can be found on the ECHA website
address: https:echa.europa.eu/de/home.
Reference service life
The reference service life of the TS Match Series door closers
depends on the traffic pattern and degree of usage of the door.
These closers are rated to EN 1154, meaning they are
designed to withstand a minimum of 500,000 cycles. The
reference service life amounts for 20 years. This corresponds
with approx. 25,000 cycles per year.
Performance data of the product with respect to its
characteristics in accordance with the relevant technical
provision which can be applied are mentioned above.
LCA: Calculation rules
Declared Unit Construction stage - Modules A4-A5
The declared unit is 1 piece of the product: TS Match Series. The construction process stage includes:
Declared unit — A4, transport to the building site;
— A5, installation into the building;
Name Value Unit
including provision of all materials, products and energy, as well
Declared unit 1 piece/product
as waste processing up to the end-of waste state or disposal of
Mass of declared Product 2.28 kg final residues during the construction process stage.
System boundary End-of-life stage– Modules C1-C4 and D
The type of EPD is: cradle to gate with options, modules C1– The end-of-life stage includes:
C4, and module D (A1–A3 + C + D and additional modules: A4 — C1, de-construction, demolition:
+ A5) — C2, transport to waste processing;
— C3, waste processing for reuse, recovery and/or recycling;
Production - Module A1-A3 — C4, disposal;
The product stage includes: including provision and all transport, provision of all materials,
— A1, raw material extraction, processing and mechanical products and related energy and water use.
treatments, processing of secondary material input (e.g.
recycling processes), — A2, transport to the manufacturer, Module D (Benefits and loads beyond the system boundary)
— A3, manufacturing and assembly including provision of all includes:
materials, products and energy, as well as waste processing up — D, recycling potentials, expressed as net impacts and
to the end-of waste state. benefits.
2 Environmental Product Declaration - dormakaba - Rack and pinion door closer TS Match and TS Match X
Geographic Representativeness Comparability
Land or region, in which the declared product system is Basically, a comparison or an evaluation of EPD data is only
manufactured, used or handled at the end of the product´s possible if all the data sets to be compared were created
lifespan: Singapore according to EN 15804 and the building context, respectively
the product-specific characteristics of performance, are taken
into account.
LCA: Scenarios and additional technical information
End of life (C1-C4)
Characteristic product properties of biogenic carbon
C1: The product dismantling from the building is done manually
Name ValueUnit
without environmental burden.
kg
Biogenic carbon content in product 0.01 C2: Transport to waste treatment at end of life is 50km.
C
Name Value Unit
Biogenic carbon content in accompanying kg
0.08 Collected separately waste type 2.05 kg
packaging C
Recycling 1.85 kg
Note: 1 kg of biogenic carbon is equivalent to 44/12 kg of CO .
2 Energy recovery 0.0307 kg
Final deposition 0,168 kg
Additional technical information for the declared modules.
Reuse, recovery and/or recycling potentials (D), relevant
Transport to the building site (A4) scenario information
Name Value Unit Name Value Unit
Litres of fuel per 1 kg (truck) 0.00276l/100km Recycling 100 %
Transport distance (truck) 750 km
Capacity utilisation (including empty runs)
55 %
average
Transport distance (ship) 17300 km
3 Environmental Product Declaration - dormakaba - Rack and pinion door closer TS Match and TS Match X
LCA: Results
DESCRIPTION OF THE SYSTEM BOUNDARY (X = INCLUDED IN LCA; MND = MODULE OR INDICATOR NOT DECLARED; MNR
= MODULE NOT RELEVANT)
Benefits and
Construction loads beyond
Product stage Use stage End of life stage
process stage the system
boundaries
la ire ta m w a Ry lp p u s tro p s n a rT g n iru tc a fu n a M e h t m o rf tro p s n a rTe tis e h t o t e ta g y lb m e s s A e s U e c n a n e tn ia M ria p e R tn e m e c a lp e R tn e m h s ib ru fe R y g re n e la n o ita re p Oe s u re ta w la n o ita re p Oe s u n o itc u rts n o c -e Dn o itilo m e d tro p s n a rT g n is s e c o rp e ts a W la s o p s iD -e s u e R-y re v o c e R-g n ilc y c e Rla itn e to p
A1 A2 A3 A4 A5 B1 B2 B3 B4 B5 B6 B7 C1 C2 C3 C4 D
X X X X X MND MND MNR MNR MNR MND MND X X X X X
RESULTS OF THE LCA - ENVIRONMENTAL IMPACT according to EN 15804+A2: 1 door closer
Parameter Unit A1-A3 A4 A5 C1 C2 C3 C4 D
GWP-total kg CO 2 eq 2.43E+01 2.79E-01 3.26E-01 0 9E-03 7.8E-02 3E-03 -6.48E+00
GWP-fossil kg CO 2 eq 2.47E+01 2.72E-01 8E-03 0 9E-03 7.8E-02 3E-03 -6.46E+00
GWP-biogenic kg CO 2 eq -3.86E-01 7E-03 3.17E-01 0 3.96E-04 1.82E-06 8.73E-06 -2E-02
GWP-luluc kg CO 2 eq 7.01E-03 6.06E-06 5.36E-06 0 2.04E-07 4.41E-06 7.35E-06 -9.58E-04
ODP kg CFC11 eq 2.45E-11 2.73E-17 5.87E-17 0 9.05E-19 3.94E-17 9.47E-18 -4.85E-11
AP mol H+ eq 1.27E-01 5E-03 9.12E-05 0 8.58E-06 1.39E-05 1.83E-05 -2.4E-02
EP-freshwater kg P eq 1.4E-05 5.96E-08 1.15E-08 0 1.84E-09 6.28E-09 4.39E-09 -3.41E-06
EP-marine kg N eq 2.02E-02 1E-03 3.29E-05 0 2.73E-06 3.13E-06 4.72E-06 -3E-03
EP-terrestrial mol N eq 2.14E-01 1.4E-02 4.11E-04 0 3.04E-05 6.33E-05 5.18E-05 -3.4E-02
kg NMVOC
POCP 6.05E-02 4E-03 8.73E-05 0 7.72E-06 8.67E-06 1.43E-05 -1E-02
eq
ADPE kg Sb eq 1.41E-04 7.6E-09 9.27E-10 0 2.57E-10 5.4E-10 2.29E-10 -2.91E-05
ADPF MJ 2.47E+02 3.59E+00 1.03E-01 0 1.22E-01 3.6E-02 3.4E-02 -9.05E+01
m3 world eq
WDP 3.63E+00 5.12E-04 4E-02 0 1.68E-05 8E-03 2.68E-04 -3.07E-01
deprived
GWP = Global warming potential; ODP = Depletion potential of the stratospheric ozone layer; AP = Acidification potential of land and water; EP =
Eutrophication potential; POCP = Formation potential of tropospheric ozone photochemical oxidants; ADPE = Abiotic depletion potential for non-fossil
resources; ADPF = Abiotic depletion potential for fossil resources; WDP = Water (user) deprivation potential)
RESULTS OF THE LCA - INDICATORS TO DESCRIBE RESOURCE USE according to EN 15804+A2: 1 door closer
Parameter Unit A1-A3 A4 A5 C1 C2 C3 C4 D
PERE MJ 2.35E+01 1.2E-02 2.78E+00 0 3.83E-04 2.19E-01 4E-03 -4.13E+01
PERM MJ 2.97E+00 0 -2.76E+00 0 0 -2.1E-01 0 0
PERT MJ 2.64E+01 1.2E-02 1.9E-02 0 3.83E-04 9E-03 4E-03 -4.13E+01
PENRE MJ 2.46E+02 3.59E+00 1.03E-01 0 1.22E-01 1.1E+00 3.4E-02 -9.06E+01
PENRM MJ 1.07E+00 0 0 0 0 -1.07E+00 0 0
PENRT MJ 2.47E+02 3.59E+00 1.03E-01 0 1.22E-01 3.6E-02 3.4E-02 -9.06E+01
SM kg 6.5E-01 0 0 0 0 0 0 0
RSF MJ 0 0 0 0 0 0 0 0
NRSF MJ 0 0 0 0 0 0 0 0
FW m3 9.6E-02 2.08E-05 9.51E-04 0 6.88E-07 1.91E-04 8.45E-06 -7.3E-02
PERE = Use of renewable primary energy excluding renewable primary energy resources used as raw materials; PERM = Use of renewable primary
energy resources used as raw materials; PERT = Total use of renewable primary energy resources; PENRE = Use of non-renewable primary energy
excluding non-renewable primary energy resources used as raw materials; PENRM = Use of non-renewable primary energy resources used as raw
materials; PENRT = Total use of non-renewable primary energy resources; SM = Use of secondary material; RSF = Use of renewable secondary fuels;
NRSF = Use of non-renewable secondary fuels; FW = Use of net fresh water
RESULTS OF THE LCA – WASTE CATEGORIES AND OUTPUT FLOWS according to EN 15804+A2:
1 door closer
Parameter Unit A1-A3 A4 A5 C1 C2 C3 C4 D
HWD kg 4.31E-07 3.5E-10 1.52E-10 0 1.18E-11 1.38E-10 5.11E-10 -5.88E-07
NHWD kg 3.79E+00 3.67E-04 1E-02 0 1.24E-05 8E-03 1.69E-01 -1.57E+00
RWD kg 1.54E-03 3.92E-06 5.4E-06 0 1.31E-07 1.34E-06 3.82E-07 -1E-02
CRU kg 0 0 0 0 0 0 0 0
MFR kg 0 0 0 0 0 1.85E+00 0 0
MER kg 0 0 0 0 0 0 0 0
EEE MJ 0 0 4.93E-01 0 0 0 0 0
EET MJ 0 0 8.94E-01 0 0 0 0 0
HWD = Hazardous waste disposed; NHWD = Non-hazardous waste disposed; RWD = Radioactive waste disposed; CRU = Components for re-use;
MFR = Materials for recycling; MER = Materials for energy recovery; EEE = Exported electrical energy; EET = Exported thermal energy
4 Environmental Product Declaration - dormakaba - Rack and pinion door closer TS Match and TS Match X
RESULTS OF THE LCA – additional impact categories according to EN 15804+A2-optional:
1 door closer
Parameter Unit A1-A3 A4 A5 C1 C2 C3 C4 D
Disease
PM 3.56E-06 8.19E-08 5.05E-10 0 4.51E-11 1.77E-10 2.27E-10 -3.84E-07
incidence
IR kBq U235 eq 2.31E-01 5.62E-04 8.36E-04 0 1.87E-05 1.21E-04 3.93E-05 -1.99E+00
ETP-fw CTUe 8.43E+01 2.54E+00 4.9E-02 0 8.6E-02 1.4E-02 1.9E-02 -3.29E+01
HTP-c CTUh 8.91E-09 4.78E-11 2.58E-12 0 1.62E-12 1.18E-12 2.84E-12 -1.25E-09
HTP-nc CTUh 2.83E-07 2.14E-09 1.12E-10 0 6.93E-11 1.19E-10 3.13E-10 -2.59E-08
SQP SQP 5.87E+01 9E-03 2.7E-02 0 3.12E-04 1.1E-02 7E-03 -2.54E+00
PM = Potential incidence of disease due to PM emissions; IR = Potential Human exposure efficiency relative to U235; ETP-fw = Potential comparative
Toxic Unit for ecosystems; HTP-c = Potential comparative Toxic Unit for humans (cancerogenic); HTP-nc = Potential comparative Toxic Unit for humans
(not cancerogenic); SQP = Potential soil quality index
Disclaimer 1 – for the indicator “Potential Human exposure efficiency relative to U235”. This impact category deals mainly with the
eventual impact of low-dose ionizing radiation on human health of the nuclear fuel cycle. It does not consider effects due to possible
nuclear accidents, occupational exposure or radioactive waste disposal in underground facilities. Potential ionizing radiation from the
soil, radon and from some construction materials is also not measured by this indicator.
Disclaimer 2 – for the indicators “abiotic depletion potential for non-fossil resources”, “abiotic depletion potential for fossil resources”,
“water (user) deprivation potential, deprivation-weighted water consumption”, “potential comparative toxic unit for ecosystems”,
“potential comparative toxic unit for humans – cancerogenic”, “Potential comparative toxic unit for humans - not cancerogenic”,
“potential soil quality index”. The results of this environmental impact indicator shall be used with care as the uncertainties on these
results are high as there is limited experience with the indicator.
References
EN 1154 GaBi ts software
EN 1154-2003; Building hardware - Controlled door closing Sphera Solutions GmbH
devices - Requirements and test methods Gabi Software System and Database for Life Cycle Engineering
1992-2020 Version 10.0.0.71
EN 15804 University of Stuttgart Leinfelden-Echterdingen
EN 15804+A2:2019+AC:2021, Sustainability of
construction works — Environmental Product GaBi ts documentation
Declarations — Core rules for the product category of GaBi life cycle inventory data documentation
construction products (https://www.gabi-software.com/support/gabi/gabidatabase-
2020-lci-documentation/)
ISO 14025
DIN EN ISO 14025:201110, Environmental labels and LCA-tool dormakaba
declarations — Type III environmental declarations — LCA tool IBU-DOR-202104-LT1-EN, version 1.0, 2021.
Principles and procedures Developed by Sphera Solutions GmbH
REACH Regulation 1907/2006/EC PCR Part A
Regulation (EC) No 1907/2006 of the European PCR – Part A: Calculation Rules for the Life Cycle Assessment
Parliament and of the Council on the Registration, and Requirements on the Project Re-port according to EN
Evaluation, Authorisation and Restriction of Chemicals 15804+A2:2019, Version 1.0, 2020, Institut Bauen und Umwelt
(REACH) e.V., www.ibu-epd.com
Further References PCR Part B
PCR – Part B: Requirements on the EPD for Building Hardware
IBU 2021 product, version 1.2, Institut Bauen und Umwelt e.V., www.ibu-
Institut Bauen und Umwelt e.V.: General Instructions for the epd.com, 2017
EPDs programme of Institut Bauen und Umwelt e.V. Version
2.0., Berlin: Institut Bauen und Umwelt e.V., 2021. www.ibu-
epd.com
5 Environmental Product Declaration - dormakaba - Rack and pinion door closer TS Match and TS Match X
Publisher
Institut Bauen und Umwelt e.V. +49 (0)30 3087748- 0
Hegelplatz 1 info@ibu-epd.com
10117 Berlin www.ibu-epd.com
Germany
Programme holder
Institut Bauen und Umwelt e.V. +49 (0)30 3087748- 0
Hegelplatz 1 info@ibu-epd.com
10117 Berlin www.ibu-epd.com
Germany
Author of the Life Cycle Assessment
Sphera Solutions GmbH +49 711 341817-0
Hauptstraße 111- 113 info@sphera.com
70771 Leinfelden-Echterdingen www.sphera.com
Germany
Owner of the Declaration
dormakaba International Holding GmbH +49 2333 793-0
DORMA Platz 1 info.de@dormakaba.com
58256 Ennepetal www.dormakaba.com
Germany
6 Environmental Product Declaration - dormakaba - Rack and pinion door closer TS Match and TS Match X
