ENVIRONMENTAL PRODUCT DECLARATION
as per ISO 14025 and EN 15804+A2
Owner of the Declaration dormakaba International Holding GmbH
Publisher Institut Bauen und Umwelt e.V. (IBU)
Programme holder Institut Bauen und Umwelt e.V. (IBU)
Declaration number EPD-DOR-20210340-CBA7-EN
Issue date 04.05.2022
Valid to 03.05.2027
BEST 9K Cylindrical Series
dormakaba
www.ibu-epd.com | https://epd-online.com
General Information
dormakaba BEST 9K Cylindrical Series
Programme holder Owner of the declaration
IBU – Institut Bauen und Umwelt e.V. dormakaba International Holding GmbH
Hegelplatz 1 DORMA Platz 1
10117 Berlin 58256 Ennepetal
Germany Germany
Declaration number Declared product / declared unit
EPD-DOR-20210340-CBA7-EN 1 cylindrical lock (1 piece) of the BEST 9K Series.
This declaration is based on the product category rules: Scope:
Building Hardware products, 01.08.2021 This Environmental Product Declaration refers to a specific lock
(PCR checked and approved by the SVR) manufactured by dormakaba. The production site is located in Indianapolis
(USA).
Issue date The data represents the year 2020.
The owner of the declaration shall be liable for the underlying information
04.05.2022
and evidence; the IBU shall not be liable with respect to manufacturer
information, life cycle assessment data and evidences.
Valid to
The EPD was created according to the specifications of EN 15804+A2. In
03.05.2027 the following, the standard will be simplified as EN 15804.
Verification
The standard EN 15804 serves as the core PCR
Independent verification of the declaration and data according to ISO
14025:2011
internally X externally
Dipl.-Ing. Hans Peters
(Chairman of Institut Bauen und Umwelt e.V.)
Florian Pronold Dr.-Ing. Wolfram Trinius,
(Managing Director Institut Bauen und Umwelt e.V.) (Independent verifier)
1 Environmental Product Declaration - dormakaba - BEST 9K Cylindrical Series
Product
Product description/Product definition
Quick installation, proven reliability and enhanced safety all
make the 9K the grade 1 cylindrical lock of choice for many. But
its wide compatibility with most large format interchangeable
cores, regardless of brand, make it a legend. Whether you want
to upgrade old hardware or fit out a new facility, the 9K is a
great match. For the use and application of the product the
respective national provisions at the place of use apply. The
standards which can be applied are the following:
• ANSI/BHMA A156.2
• ANSI A117.1
• Florida Building Code compliant
• California State Fire Marshal compliant
• BAA & TAA compliant
• UL listed
Application
The BEST 9K series can be used for following building types:
• Learning and higher education
• Healthcare
• Government
• Retail and commercial
• Multifamily
• Hospitality
Technical Data
The lock has following technical properties:
Performance data of the product with respect to its
characteristics in accordance with the relevant technical
provision which can be applied are mentioned above.
Base materials/Ancillary materials
The major material compositions including the packaging of the
product are listed below:
Name Value Unit
Zinc 44 %
Steel 27 %
Paper 9 %
Electronics 8 %
Stainless steel 7 %
Brass 4 %
Others 1 %
2 Environmental Product Declaration - dormakaba - BEST 9K Cylindrical Series
The product/s include/s partial articles which contain The Candidate List can be found on the ECHA website
substances listed in the Candidate List of REACH Regulation address: https://echa.europa.eu/de/home.
1907/2006/EC (date: 17.01.2022) exceeding 0.1 percentage by
mass: yes Reference service life
The reference service life of the 9K Series cylindrical lock
• Lead (Pb): 7439-92-1 (CAS-No.) is included in some of
depends on the traffic pattern and degree of usage of the door.
the alloys used. The concentration of lead in each
These locks are rated to ANSI Grade 1, meaning they are
individual alloy does not exceed 4.0% (by mass).
designed to withstand a minimum of 1,000,000 cycles.
However, the 9K Series cylindrical lock has to be independently
tested to surpass 65,000,000 cycles.
LCA: Calculation rules
to the end-of waste state or disposal of final residues during the
Declared Unit construction process stage.
The declared unit is 1 piece of the product: BEST 9K Cylindrical
lock. End-of-life stage– Modules C1-C4 and D
Name Value Unit The end-of-life stage includes:
Declared unit 1 piece/product — C1, de-construction, demolition:
— C2, transport to waste processing;
Mass of declared Product 2.08 kg
— C3, waste processing for reuse, recovery and/or recycling;
— C4, disposal; including provision and all transport, provision
System boundary
of all materials, products and related energy and water use.
The type of EPD is: cradle to gate with options,
- Module D (Benefits and loads beyond the system boundary)
modules C1–C4, and module D
includes:
(A1–A3 + C + D and additional modules: A4 + A5)
— D, recycling potentials, expressed as net impacts and
benefits.
Production - Module A1-A3
The product stage includes: Geographic Representativeness
— A1, raw material extraction, processing and mechanical Land or region, in which the declared product system is
treatments, processing of secondary material input (e.g. manufactured, used or handled at the end of the product´s
recycling processes), lifespan: United States
— A2, transport to the manufacturer,
— A3, manufacturing and assembly including provision of all
materials, products and energy, as well as waste processing up Comparability
to the end-of waste state. Basically, a comparison or an evaluation of EPD data is only
possible if all the data sets to be compared were created
Construction stage - Modules A4-A5 according to EN 15804 and the building context, respectively
The construction process stage includes: the product-specific characteristics of performance, are taken
— A4, transport to the building site; into account.
— A5, installation into the building; including provision of all
materials, products and energy, as well as waste processing up
LCA: Scenarios and additional technical information
Name Value Unit
Characteristic product properties of biogenic carbon
Electricity consumption for 1 year 21,9 kWh
Information on describing the biogenic Carbon Content at Power consumption "on mode" 60 W
factory gate
Hours per day in use "on mode" 1 h
Name ValueUnit
Power consumption "standby mode" 0 W
Biogenic carbon content in accompanying kg
0.01 Hours per day in use "standby mode" 23 h
packaging C
End of life (C1-C4)
C1: The product dismantling from the building is done manually
without environmental burden.
Transport to the building site (A4)
C2: Transport to waste treatment at end of life is 50km.
Name Value Unit
Name Value Unit
Litres of fuel per 1 kg (truck) 0.00276l/100km
Collected separately waste type 1.9 kg
Transport distance (truck) 1500 km
Recycling 1.75 kg
Capacity utilisation (including empty runs)
55 % Energy recovery 0.003 kg
average
Final deposition 0,152 kg
Transport distance (ship) 10000 km
Reuse, recovery and/or recycling potentials (D), relevant
Operational energy use (B6)
scenario information
Name Value Unit
Collection rate is 100%.
3 Environmental Product Declaration - dormakaba - BEST 9K Cylindrical Series
LCA: Results
DESCRIPTION OF THE SYSTEM BOUNDARY (X = INCLUDED IN LCA; MND = MODULE OR INDICATOR NOT DECLARED; MNR
= MODULE NOT RELEVANT)
Benefits and
Construction loads beyond
Product stage Use stage End of life stage
process stage the system
boundaries
la ire ta m w a Ry lp p u s tro p s n a rT g n iru tc a fu n a M e h t m o rf tro p s n a rTe tis e h t o t e ta g y lb m e s s A e s U e c n a n e tn ia M ria p e R tn e m e c a lp e R tn e m h s ib ru fe R y g re n e la n o ita re p Oe s u re ta w la n o ita re p Oe s u n o itc u rts n o c -e Dn o itilo m e d tro p s n a rT g n is s e c o rp e ts a W la s o p s iD -e s u e R-y re v o c e R-g n ilc y c e Rla itn e to p
A1 A2 A3 A4 A5 B1 B2 B3 B4 B5 B6 B7 C1 C2 C3 C4 D
X X X X X MND MND MNR MNR MNR X MND X X X X X
RESULTS OF THE LCA - ENVIRONMENTAL IMPACT according to EN 15804+A2: 1 cylindrical lock
Parameter Unit A1-A3 A4 A5 B6 C1 C2 C3 C4 D
GWP-total kg CO 2 eq 5.74E+00 3.41E-01 2.52E-01 1.23E+02 0 8E-03 8E-03 2E-03 -4.08E+00
GWP-fossil kg CO 2 eq 6.01E+00 3.29E-01 6E-03 1.23E+02 0 8E-03 8E-03 2E-03 -4.07E+00
GWP-biogenic kg CO 2 eq -2.72E-01 1.2E-02 2.46E-01 2.7E-02 0 3.66E-04 1.78E-07 7.88E-06 -6E-03
GWP-luluc kg CO 2 eq 6.6E-03 7.61E-06 4.15E-06 3.7E-02 0 1.88E-07 4.31E-07 6.64E-06 -3E-03
ODP kg CFC11 eq 1.23E-11 3.4E-17 4.55E-17 4.33E-13 0 8.35E-19 3.85E-18 8.55E-18 -1.63E-13
AP mol H+ eq 2.4E-02 3E-03 7.07E-05 1.99E-01 0 7.92E-06 1.36E-06 1.65E-05 -1.8E-02
EP-freshwater kg P eq 2.23E-05 7.11E-08 8.9E-09 6.72E-05 0 1.69E-09 6.13E-10 3.96E-09 -9.51E-06
EP-marine kg N eq 4.33E-03 7.45E-04 2.55E-05 4.3E-02 0 2.52E-06 3.06E-07 4.26E-06 -3E-03
EP-terrestrial mol N eq 4.11E-02 8E-03 3.18E-04 4.57E-01 0 2.8E-05 6.18E-06 4.68E-05 -2.7E-02
kg NMVOC
POCP 1.19E-02 2E-03 6.77E-05 1.22E-01 0 7.12E-06 8.47E-07 1.29E-05 -9E-03
eq
ADPE kg Sb eq 4.02E-03 9.57E-09 7.18E-10 2.45E-05 0 2.37E-10 5.27E-11 2.07E-10 -1E-03
ADPF MJ 8.21E+01 4.52E+00 8E-02 1.99E+03 0 1.12E-01 4E-03 3E-02 -4.96E+01
m3 world eq
WDP 1.9E+00 6.33E-04 3.1E-02 2.38E+01 0 1.55E-05 7.8E-04 2.42E-04 -8.83E-01
deprived
GWP = Global warming potential; ODP = Depletion potential of the stratospheric ozone layer; AP = Acidification potential of land and water; EP =
Eutrophication potential; POCP = Formation potential of tropospheric ozone photochemical oxidants; ADPE = Abiotic depletion potential for non-fossil
resources; ADPF = Abiotic depletion potential for fossil resources; WDP = Water (user) deprivation potential)
RESULTS OF THE LCA - INDICATORS TO DESCRIBE RESOURCE USE according to EN 15804+A2: 1 cylindrical lock
Parameter Unit A1-A3 A4 A5 B6 C1 C2 C3 C4 D
PERE MJ 3.03E+01 1.4E-02 2.15E+00 3.15E+02 0 3.54E-04 2.5E-02 4E-03 -9.39E+00
PERM MJ 2.16E+00 0 -2.14E+00 0 0 0 -2.4E-02 0 0
PERT MJ 3.25E+01 1.4E-02 1.4E-02 3.15E+02 0 3.54E-04 9.19E-04 4E-03 -9.39E+00
PENRE MJ 8.21E+01 4.53E+00 8E-02 1.99E+03 0 1.12E-01 6.1E-02 3E-02 -4.96E+01
PENRM MJ 5.8E-02 0 0 0 0 0 -5.8E-02 0 0
PENRT MJ 8.22E+01 4.53E+00 8E-02 1.99E+03 0 1.12E-01 4E-03 3E-02 -4.96E+01
SM kg 4.8E-01 0 0 0 0 0 0 0 0
RSF MJ 0 0 0 0 0 0 0 0 0
NRSF MJ 0 0 0 0 0 0 0 0 0
FW m3 5E-02 2.58E-05 7.37E-04 7.28E-01 0 6.35E-07 1.87E-05 7.63E-06 -3E-02
PERE = Use of renewable primary energy excluding renewable primary energy resources used as raw materials; PERM = Use of renewable primary
energy resources used as raw materials; PERT = Total use of renewable primary energy resources; PENRE = Use of non-renewable primary energy
excluding non-renewable primary energy resources used as raw materials; PENRM = Use of non-renewable primary energy resources used as raw
materials; PENRT = Total use of non-renewable primary energy resources; SM = Use of secondary material; RSF = Use of renewable secondary fuels;
NRSF = Use of non-renewable secondary fuels; FW = Use of net fresh water
RESULTS OF THE LCA – WASTE CATEGORIES AND OUTPUT FLOWS according to EN 15804+A2:
1 cylindrical lock
Parameter Unit A1-A3 A4 A5 B6 C1 C2 C3 C4 D
HWD kg 2.5E-07 4.4E-10 1.17E-10 7.66E-07 0 1.09E-11 1.35E-11 4.61E-10 -1.77E-06
NHWD kg 4.95E-01 4.63E-04 8E-03 6.18E-01 0 1.15E-05 7.92E-04 1.52E-01 9.4E-02
RWD kg 6.7E-03 4.89E-06 4.19E-06 1.77E-01 0 1.21E-07 1.31E-07 3.44E-07 -2E-03
CRU kg 0 0 0 0 0 0 0 0 0
MFR kg 0 0 0 0 0 0 1.74E+00 0 0
MER kg 0 0 0 0 0 0 0 0 0
EEE MJ 0 0 3.82E-01 0 0 0 0 0 0
EET MJ 0 0 6.92E-01 0 0 0 0 0 0
HWD = Hazardous waste disposed; NHWD = Non-hazardous waste disposed; RWD = Radioactive waste disposed; CRU = Components for re-use;
MFR = Materials for recycling; MER = Materials for energy recovery; EEE = Exported electrical energy; EET = Exported thermal energy
4 Environmental Product Declaration - dormakaba - BEST 9K Cylindrical Series
RESULTS OF THE LCA – additional impact categories according to EN 15804+A2-optional:
1 cylindrical lock
Parameter Unit A1-A3 A4 A5 B6 C1 C2 C3 C4 D
Disease
PM 2.78E-07 4.42E-08 3.92E-10 1.78E-06 0 4.16E-11 1.73E-11 2.05E-10 -2.5E-07
incidence
IR kBq U235 eq 6.83E-01 7E-04 6.48E-04 1.47E+01 0 1.72E-05 1.18E-05 3.54E-05 -2.29E-01
ETP-fw CTUe 3.81E+01 3.2E+00 3.8E-02 5.94E+02 0 8E-02 1E-03 1.7E-02 -2.08E+01
HTP-c CTUh 2.23E-07 6.03E-11 2E-12 1.28E-08 0 1.5E-12 1.15E-13 2.56E-12 1.1E-08
HTP-nc CTUh 4.6E-07 2.63E-09 8.67E-11 4.83E-07 0 6.4E-11 1.16E-11 2.82E-10 1.38E-06
SQP SQP 5.62E+01 1.2E-02 2.1E-02 1.82E+02 0 2.88E-04 1E-03 6E-03 -2.89E+00
PM = Potential incidence of disease due to PM emissions; IR = Potential Human exposure efficiency relative to U235; ETP-fw = Potential comparative
Toxic Unit for ecosystems; HTP-c = Potential comparative Toxic Unit for humans (cancerogenic); HTP-nc = Potential comparative Toxic Unit for humans
(not cancerogenic); SQP = Potential soil quality index
Disclaimer 1 – for the indicator “Potential Human exposure efficiency relative to U235”. This impact category deals mainly with the
eventual impact of low-dose ionizing radiation on human health of the nuclear fuel cycle. It does not consider effects due to possible
nuclear accidents, occupational exposure or radioactive waste disposal in underground facilities. Potential ionizing radiation from the
soil, radon and from some construction materials is also not measured by this indicator.
Disclaimer 2 – for the indicators “abiotic depletion potential for non-fossil resources”, “abiotic depletion potential for fossil resources”,
“water (user) deprivation potential, deprivation-weighted water consumption”, “potential comparative toxic unit for ecosystems”,
“potential comparative toxic unit for humans – cancerogenic”, “Potential comparative toxic unit for humans - not cancerogenic”,
“potential soil quality index”. The results of this environmental impact indicator shall be used with care as the uncertainties on these
results are high as there is limited experience with the indicator.
References
Standards
California State Fire Marshal
EN 15804 https://osfm.fire.ca.gov/.
EN 15804:2012+A2:2019+AC:2021, Sustainability of
construction works — Environmental Product Declarations — Florida Building Code
Core rules for the product category of construction products. https://www.floridabuilding.org/bc/bc_default.aspx.
ISO 14025 GaBi
EN ISO 14025:2011, Environmental labels and declarations — Sphera Solutions GmbH
Type III environmental declarations — Principles and Gabi Software System and Database for Life Cycle
procedures. Engineering 1992-2020
Version 10.0.0.71
IBU 2021 University of Stuttgart
Institut Bauen und Umwelt e.V.: General Instructions for the Leinfelden-Echterdingen
EPD programme of Institut Bauen und Umwelt e.V., Version
2.0, Berlin: Institut Bauen und Umwelt e.V., 2021 GaBi ts documentation
www.ibu-epd.com GaBi life cycle inventory data documentation
(https://www.gabi-software.com/support/gabi/gabidatabase-
ANSI A117.1 2020-lci-documentation/).
ANSI/ICC A117.1 - 2009, Accessible and usable buildings and
facilities. LCA-tool dormakaba
LCA-tool, EPD-DOR-202104-LT1-EN.
ANSI/BHMA A156.2 Developed by Sphera Solutions GmbH
ANSI/BHMA A156.2 - 2017, Bored & Preassembled Locks and
Latches PCR Part A
PCR – Part A: Calculation Rules for the Life Cycle Assessment
EN 15804 and Requirements on the Project Re-port
EN 15804:2019+A2, Sustainability of according to EN 15804+A2:2019, Version 1.0, 2020, Institut
construction works — Environmental Product Bauen und Umwelt e.V., www.ibu-epd.com.
Declarations — Core rules for the product category of
construction products. PCR Part B
PCR – Part B: Requirements on the EPD for Building
ISO 14025 Hardware product, 2021, Institut Bauen und
DIN EN ISO 14025:2011-10, Environmental labels and Umwelt e.V., www.ibu-epd.com.
declarations — Type III environmental declarations —
Principles and procedures. TAA
Trade Agreements Act,
Further References https://vsc.gsa.gov/administration/compDetails.cfm.
BAA UL
Buy America Act, Underwriter Laboratories, https://www.ul.com/.
https://www.gao.gov/products/105519.
5 Environmental Product Declaration - dormakaba - BEST 9K Cylindrical Series
Publisher
Institut Bauen und Umwelt e.V. +49 (0)30 3087748- 0
Hegelplatz 1 info@ibu-epd.com
10117 Berlin www.ibu-epd.com
Germany
Programme holder
Institut Bauen und Umwelt e.V. +49 (0)30 3087748- 0
Hegelplatz 1 info@ibu-epd.com
10117 Berlin www.ibu-epd.com
Germany
Author of the Life Cycle Assessment
Sphera Solutions GmbH +49 711 341817-0
Hauptstraße 111- 113 info@sphera.com
70771 Leinfelden-Echterdingen www.sphera.com
Germany
Owner of the Declaration
dormakaba International Holding GmbH +49 2333 793-0
DORMA Platz 1 info.de@dormakaba.com
58256 Ennepetal www.dormakaba.com
Germany
6 Environmental Product Declaration - dormakaba - BEST 9K Cylindrical Series
