ENVIRONMENTAL PRODUCT DECLARATION
as per ISO 14025 and EN 15804+A2
Owner of the Declaration ARGE – The European Federation of Locks and Building Hardware Manufacturers
Publisher Institut Bauen und Umwelt e.V. (IBU)
Programme holder Institut Bauen und Umwelt e.V. (IBU)
Declaration number EPD-ARG-20230552-IBG1-EN
Issue date 02.04.2024
Valid to 01.04.2029
Electromechanical building hardware and swing door operators
ARGE – The European Federation of Locks
and Building Hardware Manufacturers
This EPD is valid only for products supplied by an ARGE EPD licence holder.
www.ibu-epd.com | https://epd-online.com
1. General Information
ARGE – The European Federation of Locks Electromechanical building hardware and swing
and Building Hardware Manufacturers door operators
Programme holder Owner of the declaration
IBU – Institut Bauen und Umwelt e.V. ARGE – The European Federation of Locks and Building Hardware
Hegelplatz 1 Manufacturers
10117 Berlin Offerstraße 12
Germany 42551 Velbert
Germany
Declaration number Declared product / declared unit
EPD-ARG-20230552-IBG1-EN 1 kg of electromechanical building hardware or swing door operator
This declaration is based on the product category rules: Scope:
Building Hardware products, 01.08.2021 This ARGE EPD covers electromechanical building hardware and swing
(PCR checked and approved by the SVR) door operators used to control access on doors or gates, or enable door or
window opening and closing, as well as holding open of a door or window
by means of electrical impulse. Several products of this product group
Issue date have been assessed in separate LCA; from these LCA the worst values
per indicator and module are declared as worst-case assumption. It can
02.04.2024
therefore be used to cover all electromechanical access control devices for
doors and gates, as well as devices for opening, hold open and closing of
doors, gates and windows manufactured in Europe by ARGE member
Valid to
companies.
01.04.2029 The owner of the declaration shall be liable for the underlying information
and evidence; the IBU shall not be liable with respect to manufacturer
information, life cycle assessment data and evidences.
The EPD was created according to the specifications of EN 15804+A2. In
the following, the standard will be simplified as EN 15804.
Verification
The standard EN 15804 serves as the core PCR
Independent verification of the declaration and data according to ISO
14025:2011
Dipl.-Ing. Hans Peters internally X externally
(Chairman of Institut Bauen und Umwelt e.V.)
Florian Pronold Dr. Matthew Fishwick,
(Managing Director Institut Bauen und Umwelt e.V.) (Independent verifier)
Environmental Product Declaration - ARGE – The European Federation of Locks and Building Hardware Manufacturers - Electromechanical building hardware and swing
1 door operators
2. Product
These products are designed to be integrated into or installed
2.1 Product description/Product definition
on door, gate and window assemblies consisting of various
This ARGE EPD covers electromechanical building hardware materials and used for various applications. They may be used
and swing door operators used to control access on doors or for either interior or exterior doors, gates or windows, in
gates, or enable opening, holding open and closing of a door or accordance with manufacturer's instructions.
window, designed to potentially being integrated into access
control systems, building security and/or automation systems, 2.3 Technical Data
etc. Ideally, products should comply with a suitable technical
There are 2 principal versions of such electromechanical specification. EN 14846:2008, Building hardware – Locks and
hardware devices: latches – Electromechanically operated locks and striking
- battery-powered plates – Requirements and test methods is an example of such
- with external power supply a specification and some products will comply with it.
Performance data of such products in accordance with the
For certain products covered by this EPD the placing on the declaration of performance with respect to its essential
market in the European Union/European Free Trade characteristics according to this standard.
Association (EU/EFTA) (with the exception of Switzerland) has Performance data of other products in respect to its
to be compliant with Regulation (EU) No. 305/2011 (CPR). characteristics in accordance with the relevant technical
These products need a declaration of performance taking into provision (no CE-marking).
consideration EN 14846:2008 Building hardware – Locks and
latches – Electromechanically operated locks and striking 2.4 Delivery status
plates – Requirements and test methods and the CE-marking. The products are sold by unit. Deliveries of individual items are
possible but are an exception. Standard deliveries comprise a
In addition to such products requiring a CE-marking under EN larger quantity of electromechanical building hardware devices,
14846 all of the following products require a CE-marking as for as they are marketed as "B2B" products and not to end-users.
placing in the European Union/European Free Trade
2.5 Base materials/Ancillary materials
Association (EU/EFTA) (with the exception of Switzerland)
other legal provisions apply: Composition of product analysed for this EPD:
• Electromechanically operated locks and striking plates,
The values given in the table below are for the product
if no CE-marking is required under EN 14846:2008.
analysed for this EPD:
• Mechatronic cylinders: EN 15684:2020, Building
Name Value Unit
hardware - Mechatronic cylinders - Requirements and
test methods. Steel 71.93 %
• Mechatronic padlocks: EN 16864:2017, Building Stainless steel 20.8 %
hardware - Mechatronic padlocks - Requirements and Zamak 3.63 %
test methods.
Motor 1.37 %
• Mechatronic door furniture: EN 16867:2020+A1:2021,
PCB 1.08 %
Building hardware - Mechatronic door furniture -
Requirements and test methods. ABS 0.92 %
• Electrically controlled exit systems for use on escape Acetal 0.26 %
routes: EN 13637:2015, Building hardware - Electrically Neodymium 0.0000159 %
controlled exit systems for use on escape routes -
Steel is produced by combining iron with carbon as well as
Requirements and test methods.
other elements depending on the desired characteristics.
• Electrically powered hold-open devices for swing doors:
Components made of steel are formed by stamping or other
EN 1155:1997+A1:2002+AC:2006, Building hardware -
types of mechanical processing.
Electrically powered hold-open devices for swing doors -
Requirements and test methods.
Stainless steel is produced by combining iron with chromium
These other legal provisions which might apply for the
as well as other elements depending on the desired
electromechanical building hardware devices are:
characteristics. Components made of steel are formed by
• Directive (EU) No. 2014/35 (Low Voltage Directive stamping or other types of mechanical processing.
(LVD))
• Directive (EU) No. 2014/30 (Electromagnetic Zamak is an alloy with a base metal of zinc and alloying
Compatibility (EMC) Directive) elements of aluminium, magnesium, and copper. Components
• Directive (EU) No. 2014/53 (Radio Equipment Directive made of Zamak are die-cast.
(RED))
• Directive (EU) No. 2011/65 (Directive on the restriction Motor, PCB are electronic components, which include copper
of the use of certain hazardous substances in electrical wiring, etched copper sheets on non-conductive substrates,
and electronic equipment (RoHS Directive)) resistors, transistors, etc.
• Directive (EU) No. 2006/42 (Machinery Directive)
The respective CE-marking takes into account the proof of ABS (acrylonitrile butadiene styrene) is a terpolymer polymer
conformity with the relevant harmonised standard(s) based on made by polymerizing styrene and acrylonitrile in the presence
these legal provisions or with the legal provision itself. of polybutadiene. Components made of ABS are made by
injection moulding or other thermal forming processes.
For the application and use the respective national provisions
apply. Acetal, or polyoxymethylene (POM), is produced by
polymerisation of anhydrous formaldehyde. Components made
2.2 Application
of Acetal are formed by injection moulding or other thermal
Environmental Product Declaration - ARGE – The European Federation of Locks and Building Hardware Manufacturers - Electromechanical building hardware and swing
2 door operators
forming processes. disposal (including recycling).
Neodymium is a chemical element and Neodymium alloys, 2.10 Condition of use
used in high quality permanent magnets, consist of pure Once installed, the products shall require no servicing during
neodymium, iron, and boron. their expected service lives. There shall be no consumption of
water linked to their use, and they shall not cause any
Battery (in case of battery-powered electromechanical emissions.
devices): AA 1.5V Lithium or similar.
2.11 Environment and health during use
1) This product/article/at least one partial article contains No environmental damage or health risks are to be expected
substances listed in the ECHA candidate list (date: 14.06.2023) during normal conditions of use.
exceeding 0.1 percentage by mass: Certain components may
2.12 Reference service life
contain small amounts of lead (CAS no. 7439-92-1) as an
A reference service life according to ISO 15686 cannot be
alloying element.
declared.
The typical service life is 10 years under normal working
2) This product/article/at least one partial article contains other
conditions. The service life is not limited due to mechanical
cancerogenic, mutagenic, reprotoxic (CMR) substances in
obsolescence but due to outdated electronic
categories 1A or 1B which are not on the ECHA candidate list,
components/software.
exceeding 0.1 percentage by mass: no.
It is required that installation, as well as maintenance of the
product, must be done in line with instructions provided by the
3) Biocide products were added to this construction product or it
manufacturer.
has been treated with biocide products (this then concerns a
treated product as defined by the (EU) Ordinance on Biocide
2.13 Extraordinary effects
Products No. 528/2012): no.
Fire
2.6 Manufacture Certain products are suitable for use on fire resisting and/or
smoke control door/window sets according to e.g., one of the
The manufacture of an electromechanical building hardware
classes A, B, N in EN 12209. Specific needs on fire resistance
device usually follows a 3-step process:
are addressed by individual manufacturers.
1. Manufacture of the components: this step may include
surface treatment in the factory or by external Water
contractors. The declared product is intended to be used in buildings under
2. Pre-assembly of modules (in the factory). normal conditions (indoor or outdoor). It shall not emit
3. Final assembly (in the factory). hazardous substances in the event of flooding.
2.7 Environment and health during manufacturing
Mechanical destruction
Regular measurements of air quality and noise levels are
Mechanical destruction of the declared product shall not
carried out by the manufacturers, the ARGE member
materially alter its composition or have any adverse effect on
companies. The results shall be within the mandatory safety
the environment.
levels. In areas where employees are exposed to chemical
products, the required protective clothing and technical 2.14 Re-use phase
protective devices shall be provided. Regular health checks are Removal of electromechanical building hardware (for re-use or
mandatory for employees in production facilities. recycling) shall have no adverse effect on the environment.
2.8 Product processing/Installation 2.15 Disposal
The installation of the product may vary depending on the type Electromechanical building hardware components should be re-
of door, gate or window and the specific situation, but the cycled wherever possible, providing that there is no adverse
products shall not require energy consumption for installation. effect on the environment. The waste code in accordance with
the European Waste Code is 17 04 07.
2.9 Packaging
Normally, each individual product is packed in paper or 2.16 Further information
cardboard. These individual products are then packed in a Details of all types and variants can be found on the
cardboard box and stacked on wooden pallets for transport to manufacturers' websites. The respective website addresses are
the customer. available at https://arge.org.
Waste from product packaging is collected separately for waste
3. LCA: Calculation rules
Name Value Unit
3.1 Declared Unit
Declared unit 1 kg
The declared unit for all products covered by ARGE EPD is 1
Mass of assessed products 0.63 - 7.5 kg
kg (of product). Since individual products will rarely weigh
exactly 1 kg it is necessary to establish the exact weight of the Raw density 1 kg/m3
product then use this as a correction factor to determine the
true values for 1 kg of product in the tables (Section 5). 3.2 System boundary
Declared unit Type of the EPD: "cradle to gate with options, with modules C1
– C4, and module D (A1-A3, C1-C3, D and additional
modules)"
The analysis of the product life cycle includes the production
Environmental Product Declaration - ARGE – The European Federation of Locks and Building Hardware Manufacturers - Electromechanical building hardware and swing
3 door operators
and transport of the raw materials, manufacture of the product
and the packaging materials which are declared in modules A1- 3.5 Background data
A3. For life cycle modelling of the considered product, all relevant
Losses during production are considered as waste and are sent background datasets are taken from ecoinvent v3.8 (system
for recycling. No recycling processes are taken into account model: cut-off by classification).
except transport and electricity consumption for grinding the
3.6 Data quality
metals. When recycled metals are used as raw material only
their transformation process is taken into account and not the The objective of this evaluation is to evaluate the environmental
extraction of the raw material. impacts generated by the products throughout their entire life
cycles. To this end, ISO 14040, ISO 14044 and EN 15804 have
A4 module represents the transport of the finished
been met regarding the quality of data on the following different
electromechanical building hardware or swing door operator to
the installation site. criteria:
There is no waste associated with the installation of the
product. The A5 module therefore represents only the disposal Time: The life cycle inventory data used come from:
of the product packaging. • Data collected specifically for this study on the ARGE
member company's manufacturing site. Datasets are
Two alternatives are declared for the power supply: based on 1-year averaged data (time period: January
2013 to December 2013 considered representative for
• B6_1: replacement of the battery every 2 years (for
2022).
battery-powered devices)
• B6_2: energy consumption from the grid (for grid- • In the absence of collected data, generic data from the
connected devices) ecoinvent v3.8 database have been used. This is
updated regularly and is representative of current
processes (the entire database having been updated in
The End-of-Life (EoL) stages are also considered. The
2021).
transportation to the EoL disposal site is taken into account in
module C2. Module C4 covers the disposal of the Geography: Data come from the production site of the ARGE
electromechanical building hardware or swing door operator. member company. Generic data come from the ecoinvent
Module C3 covers the recycling of the individual elements database, representative for European production processes.
according to European averages, with the remaining waste
divided between incineration and landfill. Technology: Material shaping technologies are based on
Such a mixed scenario is declared due to the complex material European technology in the case of use of generic data.
mix of the product and the dependency of the EoL-route on the
EoL-route of the product the electromechanical building Several products of this product group have been assessed in
hardware or swing door operator has been integrated into. separate LCAs; from these LCA the worst values per indicator
In practice, the end of life has been modelled as follows: and module are declared as worst-case assumption.
• when a material is sent for recycling, generic transport 3.7 Period under review
and electric consumption of a shredder is taken into The data of the LCA is based on the annual production data of
account (corresponding to the process 'Grinding, an ARGE member from 2013, considered also representative
metals'). Only then, is the material considered to have for the year 2022.
attained the 'end of waste' state.
• each type of waste is modelled as a transport to the 3.8 Geographic Representativeness
treatment site with a distance of 30 km. Parts sent for Land or region, in which the declared product system is
recycling include electricity consumption (grinding) and manufactured, used or handled at the end of the product´s
a flow ('Materials for recycling, unspecified'). lifespan: Europe
3.3 Estimates and assumptions
The LCA data of the declared product had been calculated by 3.9 Allocation
the production data from one ARGE member company. This The products covered by this EPD are produced in numerous
company had been chosen by ARGE as being representative sites. The product assessed for the calculation of this EPD is
by means of its production processes and its market share. The produced by one manufacturer on its own site. All data were
product is chosen to be as representative as possible. In provided by this manufacturer of the product per unit, and then
addition, data were used from another manufacturer to consider divided by the mass of the product to give a value per kg of
battery-powered devices in order to complete the LCA results. product produced.
3.4 Cut-off criteria
In addition, a battery-powered device was considered to
The cut-off criteria considered are 1% of renewable and non- complete the evaluation. The data were provided by another
renewable primary energy usage and 1% of the total mass of manufacturer.
that unit process. The total neglected input flows per module
amount to a maximum of 5% of energy usage and mass. The assumptions relating to the EoL of the product are
described in the section System Boundaries.
For this study, all input and output flows have been considered
at 100%, including raw materials as per the product 3.10 Comparability
composition provided by the manufacturer and packaging of Basically, a comparison or an evaluation of EPD data is only
raw materials as well as the final product. Energy and water possible if all the data sets to be compared were created
consumptions have also been considered at 100% according to according to EN 15804 and the building context, respectively
the data provided. the product-specific characteristics of performance, are taken
into account.
With the approach chosen, no significant environmental
impacts are known to have been cut off. ecoinvent v3.8 (system model: cut-off by classification) has
been used as the background database.
Environmental Product Declaration - ARGE – The European Federation of Locks and Building Hardware Manufacturers - Electromechanical building hardware and swing
4 door operators
4. LCA: Scenarios and additional technical information
Characteristic product properties of biogenic carbon Energy consumption of the product (Wh) = Energy
consumption active + Energy consumption standby + Energy
Information on the biogenic carbon content at factory gate consumption off
Note: 1 kg of biogenic carbon is equivalent to 44/12 kg of CO .
2
It is assumed that, throughout its RSL (10 years), the product is
Name Value Unit active 1% of the time and is in stand-by or sleep-mode during
kg 99 % of the time (data from companies).
Biogenic carbon content in product 0
C The average power during the active time is 28.8 W (17660.16
Biogenic carbon content in accompanying kg Wh) and during stand-by is 3.6 W (218544.48 Wh). A European
0.0678
packaging C electricity mix has been taken into account for the energy
consumption.
Name Value Unit
The following information is the basis of the declared modules
Electricity consumption 236.2 kWh
within the LCA in this EPD.
Transport to the building site (A4) End of life (C1-C4)
Name Value Unit Name Value Unit
Litres of fuel 28.5 l/100km Collected separately waste type 1 kg
Transport distance 3500 km Recycling 0.241 kg
Capacity utilisation (including empty runs) 36 % Energy recovery 0.349 kg
Landfilling 0.41 kg
Installation into the building (A5)
Name Value Unit It is assumed that a 16–32-ton truck is used to transport the
product:
Material loss 0.00949 kg
- Transport to shredding facility for metal recovery: 150 km
- Transport to municipal waste incineration plant: 50 km
Reference service life - Transport to landfill: 30 km
Name Value Unit
Reuse, recovery and/or recycling potentials (D), relevant
Life Span according to the manufacturer 10 a scenario information
The service life is not limited due to mechanical obsolescence
but due to outdated electronic components/software. Module D contains the benefits and loads beyond the system
It is required that installation, as well as maintenance of the boundary related to the recycling of metals, which result from
product, must be done in line with instructions provided by the the treatment of recycled materials from the point of end-of-
manufacturer. waste status to the point of substitution (as costs) and the
substitution of primary resources (as benefits).
Operational energy use (B6)
According to EN 16710, clause 6.4.3.3: 'In module D
Two alternatives are declared for the power supply:
substitution effects are calculated only for the resulting net
• B6_1: replacement of the battery every 2 years (for output flow.
battery-powered devices)
• B6_2: energy consumption from the grid (for grid- For building hardware, the following rules apply for the
connected devices) quantification of net output flows:
When electromechanical hardware devices are battery- - all production scrap and cuttings leave modules A1-B3 as
powered, the batteries are assumed to be replaced every 2 sorted scrap without allocated burdens from primary production;
years which leads to 2 replacements of a set of 2 batteries over the corresponding amounts are declared as material for
a service life of 5 years. recycling (MFR);
- net amounts of a metal leaving the product system are
The transport of the battery is assumed to be done by truck (3.5 quantified as the material for recycling leaving modules A1-C4
tons) with a distance of 30 km. minus the input of secondary scrap (secondary material, SM) to
the product system;
The following scenario has been taken into account for the grid- - in the case of brass and zinc alloys, which are composed of
connected version: two different constituting metals, no difference shall be made
- 3 operative modes of the product: Active mode, standby and between the input of secondary constituting metals (Cu and Zn;
off Cu and Sn) and its alloys (CuZn; CuSn).
- Time share in each mode (in %) Negative net output flows have been considered in the
- Average power for each mode (in Watts) quantification of module D.
The total energy consumption during the RSL has been
calculated with the following formulas: It also includes the benefits and loads related to 'exported
energy electricity' and 'exported energy heat' resulting from the
Energy consumption mode (Wh) = Average power mode (W) energy recovery from plastic wastes in a municipal waste
* Time mode (%) * RSL * 365 * 24 incineration plant as modelled in Modules A3, A5 and C4.
Environmental Product Declaration - ARGE – The European Federation of Locks and Building Hardware Manufacturers - Electromechanical building hardware and swing
5 door operators
5. LCA: Results
In Table 1 "Description of the system boundary", the declared modules are indicated with an "X"; all modules that are not declared
within the EPD but where additional data are available are indicated with "MND". Those data can also be used for building assessment
scenarios. The values are declared with three valid digits in exponential form.
The set of characterisation factors EF3.0 has been used for the life cycle assessment.
DESCRIPTION OF THE SYSTEM BOUNDARY (X = INCLUDED IN LCA; MND = MODULE OR INDICATOR NOT DECLARED; MNR
= MODULE NOT RELEVANT)
Benefits and
Construction loads beyond
Product stage Use stage End of life stage
process stage the system
boundaries
la ire wta am R y lp p u s tro p s n a rT g n iru tc a fu n a M tro p s nm ae o rh r
T
f te tis e h t o t e ta g y lb m e s s A e s U e c n a n e tn ia M ria p e R tn e m e c a lp e R tn e m h s ib ru fe R la n o ity ag rr ee pn Oe e s u la n o ita r re et pa Ow e s u n o itc u rts n eo Dc -n o itilo m e d tro p s n a rT g n is s ee tsc ao Wrp la s o p s iD e s u e R- y re v o c e R- g n ilc y c e R- la itn e to p
A1 A2 A3 A4 A5 B1 B2 B3 B4 B5 B6 B7 C1 C2 C3 C4 D
X X X X X MND MND MNR MNR MNR X MND X X X X X
RESULTS OF THE LCA - ENVIRONMENTAL IMPACT according to EN 15804+A2: 1 kg of electromechanical building hardware
and swing door operators
Parameter Unit A1-A3 A4 A5 B6/1 B6/2 C1 C2 C3 C4 D
GWP-total kg CO2 eq 1.18E+01 6.75E-01 3.14E-01 1.48E+00 2.03E+02 0 1.86E-02 1.86E-02 4.93E-02 4.85E-01
GWP-fossil kg CO2 eq 1.2E+01 6.74E-01 2.26E-02 1.47E+00 2.03E+02 0 1.86E-02 1.85E-02 4.93E-02 4.84E-01
GWP-
biogenic
kg CO2 eq -2.69E-01 0 2.92E-01 0 0 0 0 0 0 0
GWP-luluc kg CO2 eq 2.82E-02 2.7E-04 1.8E-06 2.69E-03 5.07E-01 0 7.44E-06 3.14E-05 3.75E-06 7.47E-04
ODP kg CFC11 eq 6.48E-07 1.56E-07 1.02E-09 1.15E-07 1.05E-05 0 4.31E-09 8.96E-10 1.52E-09 3.2E-08
AP mol H+ eq 3.08E-01 1.91E-03 1.95E-05 3.07E-02 1.11E+00 0 5.28E-05 2.03E-04 4.35E-05 2.35E-02
EP-
kg P eq 1.87E-03 4.81E-06 3.74E-08 1.66E-04 2.27E-02 0 1.33E-07 1.06E-06 8.24E-08 7.47E-05
freshwater
EP-marine kg N eq 3.85E-02 3.81E-04 6.46E-06 2.35E-03 1.38E-01 0 1.05E-05 1.67E-05 1.76E-05 1.02E-03
EP-terrestrial mol N eq 2.8E-01 4.24E-03 6.99E-05 2.81E-02 1.6E+00 0 1.17E-04 1.85E-04 1.7E-04 1.4E-02
kg NMVOC
POCP 7.77E-02 1.63E-03 2.03E-05 8.53E-03 4.4E-01 0 4.5E-05 5.78E-05 4.98E-05 4.23E-03
eq
ADPE kg Sb eq 4.07E-03 2.39E-06 1.62E-08 5.7E-04 1.97E-03 0 6.59E-08 7.78E-07 2.26E-08 5.66E-04
ADPF MJ 1.29E+02 1.02E+01 6.85E-02 1.93E+01 4.27E+03 0 2.82E-01 2.38E-01 1.11E-01 6.82E+00
m3 world eq
WDP 5.06E+00 3.11E-02 3.36E-04 8.35E-01 5.07E+01 0 8.58E-04 9.87E-03 -3.16E-04 4.14E-01
deprived
GWP = Global warming potential; ODP = Depletion potential of the stratospheric ozone layer; AP = Acidification potential of land and water; EP =
Eutrophication potential; POCP = Formation potential of tropospheric ozone photochemical oxidants; ADPE = Abiotic depletion potential for non-fossil
resources; ADPF = Abiotic depletion potential for fossil resources; WDP = Water (user) deprivation potential)
RESULTS OF THE LCA - INDICATORS TO DESCRIBE RESOURCE USE according to EN 15804+A2: 1 kg of electromechanical
building hardware and swing door operators
Parameter Unit A1-A3 A4 A5 B6/1 B6/2 C1 C2 C3 C4 D
PERE MJ 2.15E+01 1.44E-01 -6.86E-01 2.56E+00 9.42E+02 0 3.96E-03 9.18E-02 6.71E-03 1.33E+00
PERM MJ 2.35E+00 0 -6.18E-01 0 0 0 0 0 0 0
PERT MJ 2.38E+01 1.44E-01 -1.3E+00 2.56E+00 9.42E+02 0 3.96E-03 9.18E-02 6.71E-03 1.33E+00
PENRE MJ 1.31E+02 1.02E+01 2.17E-01 1.93E+01 4.32E+03 0 2.82E-01 2.39E-01 1.11E-01 6.85E+00
PENRM MJ 1.43E+00 0 -1.48E-01 0 0 0 0 0 0 0
PENRT MJ 1.33E+02 1.02E+01 6.85E-02 1.93E+01 4.32E+03 0 2.82E-01 2.39E-01 1.11E-01 6.85E+00
SM kg 4.47E-01 0 0 0 0 0 0 0 0 0
RSF MJ 0 0 0 0 0 0 0 0 0 0
NRSF MJ 0 0 0 0 0 0 0 0 0 0
FW m3 1.62E-01 1.08E-03 5.13E-05 1.88E-02 2.84E+00 0 2.99E-05 2.75E-04 2.23E-04 6.66E-03
PERE = Use of renewable primary energy excluding renewable primary energy resources used as raw materials; PERM = Use of renewable primary
energy resources used as raw materials; PERT = Total use of renewable primary energy resources; PENRE = Use of non-renewable primary energy
excluding non-renewable primary energy resources used as raw materials; PENRM = Use of non-renewable primary energy resources used as raw
materials; PENRT = Total use of non-renewable primary energy resources; SM = Use of secondary material; RSF = Use of renewable secondary fuels;
NRSF = Use of non-renewable secondary fuels; FW = Use of net fresh water
RESULTS OF THE LCA – WASTE CATEGORIES AND OUTPUT FLOWS according to EN 15804+A2:
1 kg of electromechanical building hardware and swing door operators
Parameter Unit A1-A3 A4 A5 B6/1 B6/2 C1 C2 C3 C4 D
HWD kg 1.47E-03 2.67E-05 2.49E-07 7.99E-04 3.41E-03 0 7.36E-07 4.47E-07 2.15E-07 1.92E-04
NHWD kg 4.71E+00 5.38E-01 4.05E-03 5.53E-01 1.72E+01 0 1.48E-02 1.37E-02 3.8E-01 1.71E-01
Environmental Product Declaration - ARGE – The European Federation of Locks and Building Hardware Manufacturers - Electromechanical building hardware and swing
6 door operators
RWD kg 2.12E-03 1.48E-04 9.43E-07 9.02E-05 5.73E-02 0 4.08E-06 1.95E-06 1.41E-06 5.49E-05
CRU kg 0 0 0 0 0 0 0 0 0 0
MFR kg 2.89E-01 0 1.61E-01 0 0 0 0 6.72E-01 0 0
MER kg 0 0 0 0 0 0 0 0 0 0
EEE MJ 0 0 0 0 0 0 0 0 0 0
EET MJ 0 0 0 0 0 0 0 0 0 0
HWD = Hazardous waste disposed; NHWD = Non-hazardous waste disposed; RWD = Radioactive waste disposed; CRU = Components for re-use;
MFR = Materials for recycling; MER = Materials for energy recovery; EEE = Exported electrical energy; EET = Exported thermal energy
RESULTS OF THE LCA – additional impact categories according to EN 15804+A2-optional:
1 kg of electromechanical building hardware and swing door operators
Parameter Unit A1-A3 A4 A5 B6/1 B6/2 C1 C2 C3 C4 D
Disease
PM 1.29E-06 5.42E-08 3.98E-10 1.34E-07 3.24E-06 0 1.49E-09 1.19E-09 1.05E-09 5.38E-08
incidence
IR kBq U235 eq 7.95E-01 4.44E-02 2.85E-04 5.64E-02 3.89E+01 0 1.22E-03 1.32E-03 5.02E-04 3.51E-02
ETP-fw CTUe 2.54E+03 8.02E+00 5.87E-02 2.18E+02 2.67E+03 0 2.21E-01 1.06E+00 5.48E+01 1.28E+02
HTP-c CTUh 6.79E-08 2.58E-10 3.64E-12 8.96E-09 8.58E-08 0 7.12E-12 2.13E-11 1.22E-11 5.6E-09
HTP-nc CTUh 3.43E-06 8.11E-09 1.44E-10 3.53E-07 2.7E-06 0 2.24E-10 5.82E-10 3.96E-10 3.81E-07
SQP SQP 1.14E+02 7.13E+00 4.58E-02 1.12E+01 8.22E+02 0 1.96E-01 7.52E-02 1.89E-01 8.77E+00
PM = Potential incidence of disease due to PM emissions; IR = Potential Human exposure efficiency relative to U235; ETP-fw = Potential comparative
Toxic Unit for ecosystems; HTP-c = Potential comparative Toxic Unit for humans (cancerogenic); HTP-nc = Potential comparative Toxic Unit for humans
(not cancerogenic); SQP = Potential soil quality index
Disclaimer 1 – for the indicator 'Potential Human exposure efficiency relative to U235'. This impact category deals mainly with the
eventual impact of low dose ionizing radiation on human health of the nuclear fuel cycle. It does not consider effects due to possible
nuclear accidents, occupational exposure nor due to radioactive waste disposal in underground facilities. Potential ionizing radiation
from the soil, from radon and from some construction materials is also not measured by this indicator.
Disclaimer 2 – for the indicators 'abiotic depletion potential for non-fossil resources', 'abiotic depletion potential for fossil resources',
'water (user) deprivation potential, deprivation-weighted water consumption', 'potential comparative toxic unit for ecosystems', 'potential
comparative toxic unit for humans – cancerogenic', 'Potential comparative toxic unit for humans - not cancerogenic', 'potential soil
quality index'. The results of this environmental impact indicator shall be used with care as the uncertainties on these results are high
or as there is limited experienced with the indicator.
6. LCA: Interpretation
The following interpretation is based on the LCA scores of one modules along the life cycle of the declared products, assuming
of the assessed products, whereas two types of power supply power supply from the grid.
have been analysed.
Figure 1 illustrates the relative contributions of the different
electricity from the grid during standby. With the exception of
the ADP elements, the production (modules A1-A3) of the
Figure 1: Environmental impacts of electromechanical electromechanical building hardware and swing door operators
building hardware and swing door operators with external has negligible impacts.
power supply along their life cycle All the other modules related to the product life cycle and
module D are not significant.
By far the largest part of environmental impact is caused by the
Environmental Product Declaration - ARGE – The European Federation of Locks and Building Hardware Manufacturers - Electromechanical building hardware and swing
7 door operators
Figure 2 illustrates the relative contributions of the different
modules along the life cycle of the battery-powered products.
Benefits and burdens beyond the system boundary (module D)
are in the order of +5 % to +15 % hence resulting in net
Figure 2: Environmental impacts of battery-powered burdens due to a negative net flow of recycled materials over
electromechanical building hardware along its life cycle the product life cycle.
The largest part of environmental impacts is caused during Several typical products (based on sales figures) have been
production (modules A1-A3); comparably small impacts are evaluated and the worst-case results are used in section 5 of
caused during the transport of the product to the construction this EPD. In chapter 2.5, the tabulated range of relative weight
site (via the manufacturer of the product, which the per material ensures that the variability of results stays within
electromechanical hardware has been integrated into). +/- 40% of the declared values (assessed for the indicators
All the other modules related to the product life cycle are not GWP, PENRT, and non-hazardous waste).
significant.
7. Requisite evidence
No testing results are required by the PCR part B.
Environmental Product Declaration - ARGE – The European Federation of Locks and Building Hardware Manufacturers - Electromechanical building hardware and swing
8 door operators
8. References
Product category rules of IBU systems for use on escape routes - Requirements and test
methods.
IBU (2021)
IBU (2021): General Instructions for the EPD Programme of the EN 13501-1
Institut Bauen und Umwelt e.V. (General Instructions for the EN 13501-1:2018, Fire classification of construction products
IBU EPD Programme). Version 2.0, Institut Bauen und Umwelt, and building elements - Part 1: Classification using data from
Berlin. reaction to fire tests.
IBU (2021) ISO 15686
IBU (2021): PCR Part A: Calculation rules for the life cycle ISO 15686:1, -2, -7 and -8. Service life planning (various parts).
assessment and requirements on the project report according
to EN 15804+A2. Version 1.3., Institut Bauen und Umwelt, Regulation No. 305/2011
Berlin. Regulation No. 305/2011 (Construction Products Regulation, or
CPR) of the European Parliament and of the European Council
IBU (2023) is a regulation of 9 March 2011 that lays down harmonised
IBU (2023): PCR Part B: Requirements on the EPD for building conditions for the marketing of construction products and
hardware products, Institut Bauen und Umwelt, Berlin. replaces Construction Products Directive (89/106/EEC).
Standards and legal documents Directive No. 2014/35
Directive No. 2014/35/EU (Low Voltage Directive, or LVD) of the
EN 15804 European Parliament and of the Council of 26 February 2014
EN 15804:2012+A2:2019+AC:2021, Sustainability of on the harmonisation of the laws of the Member States relating
construction works - Environmental product declarations - Core to the making available on the market of electrical equipment
rules for the product category of construction products. designed for use within certain voltage limits (recast).
EN 17610 Directive No. 2014/30
EN 17610:2022, Building hardware - Environmental product Directive No. 2014/30 (Electromagnetic Compatibility Directive,
declarations - Product category rules complementary to EN or EMC) of the European Parliament and of the Council of 26
15804 for building hardware. February 2014 on the harmonisation of the laws of the Member
States relating to electromagnetic compatibility.
ISO 14025
ISO 14025:2006-07, Environmental labels and declarations - Directive No. 2014/53
Type III Environmental declarations - Principles and Directive No. 2014/53 (Radio Equipment Directive, or RED) of
procedures. the European Parliament and of the Council of 16 April 2014 on
the harmonisation of the laws of the Member States relating to
ISO 14044 the making available on the market of radio equipment and
EN ISO 14044:2006-07, Environmental management - Life repealing Directive 1999/5.
cycle assessment - Requirements and guidance (ISO
14044:2006); German and English versions EN ISO Directive No. 2011/65
14044:2006. Directive No. 2011/65 (RoHS) of the European Parliament and
of the Council of 8 June 2011 on the restriction of the use of
EN 15684 certain hazardous substances in electrical and electronic
EN 15684:2020, Building hardware - Mechatronic cylinders - equipment.
Requirements and test methods.
Directive No. 2006/42
EN 16864 Directive No. 2006/42 (Machinery Directive) of the European
EN 16864:2017, Building hardware - Mechatronic padlocks - Parliament and of the Council of 17 May 2006 on machinery,
Requirements and test methods. and amending Directive 95/16/EC (recast).
EN 16867 ECHA candidate list
EN 16867:2020+A1:2021, Building hardware - Mechatronic Candidate List of substances of very high concern for
door furniture - Requirements and test methods. Authorisation, published in accordance with Article 59(10) of the
REACH Regulation. European Chemicals Agency, Brussels.
EN 14846
EN 14846:2008, Building hardware - Locks and latches - Ordinance on Biocide Products No. 528/2012
Electromechanically operated locks and striking plates - REGULATION (EU) No 528/2012 OF THE EUROPEAN
Requirements and test methods. PARLIAMENT AND OF THE COUNCIL of 22 May 2012
concerning the making available on the market and use of
EN 1155 biocidal products.
EN 1155:1997+A1:2002+AC:2006, Electrically powered hold-
open devices for swing doors: Building hardware - Electrically European List of Waste
powered hold-open devices for swing doors - Requirements Commission Decision of 3 May 2000 replacing Decision
and test methods. 94/3/EC establishing a list of wastes pursuant to Article 1(a) of
Council Directive 75/442/EEC on waste and Council Decision
EN 13637 94/904/EC establishing a list of hazardous waste pursuant to
EN 13637:2015, Building hardware - Electrically controlled exit Article 1(4) of Council Directive 91/689/EEC on hazardous
Environmental Product Declaration - ARGE – The European Federation of Locks and Building Hardware Manufacturers - Electromechanical building hardware and swing
9 door operators
waste (notified under document number C(2000) 1147). Lebenszyklusanalysen nach Bewertungssystem Nachhaltiges
Bauen (BNB). Version vom 24.10.2017, Bundesinstitut für Bau-,
Additional references Stadt- und Raumforschung, Berlin.
BBSR 2017 ecoinvent v3.8
BBSR (2017): Nutzungsdauer von Bauteilen in http://www.ecoinvent.org
Environmental Product Declaration - ARGE – The European Federation of Locks and Building Hardware Manufacturers - Electromechanical building hardware and swing
10 door operators
Publisher
Institut Bauen und Umwelt e.V. +49 (0)30 3087748- 0
Hegelplatz 1 info@ibu-epd.com
10117 Berlin www.ibu-epd.com
Germany
Programme holder
Institut Bauen und Umwelt e.V. +49 (0)30 3087748- 0
Hegelplatz 1 info@ibu-epd.com
10117 Berlin www.ibu-epd.com
Germany
Author of the Life Cycle Assessment
Dr. Frank Werner - Umwelt & Entwicklung + 41 (0)44 241 39 06
Kammelenbergstrasse 30 frank@frankwerner.ch
9011 St. Gallen http://www.frankwerner.ch/
Switzerland
Owner of the Declaration
ARGE – The European Federation of Locks and +49 (0)2051 9506 15
Building Hardware Manufacturers mail@arge.org
Offerstraße 12 www.arge.org
42551 Velbert
Germany
Environmental Product Declaration - ARGE – The European Federation of Locks and Building Hardware Manufacturers - Electromechanical building hardware and swing
11 door operators
