ENVIRONMENTAL PRODUCT DECLARATION
as per ISO 14025 and EN 15804+A2
Owner of the Declaration Adolf Würth GmbH & Co. KG
Publisher Institut Bauen und Umwelt e.V. (IBU)
Programme holder Institut Bauen und Umwelt e.V. (IBU)
Declaration number EPD-AWU-20230267-IBD1-EN
Issue date 12.09.2023
Valid to 12.09.2027
flexen® Exzenterblock Compact
Adolf Würth GmbH & Co. KG
www.ibu-epd.com | https://epd-online.com
1. General Information
Adolf Würth GmbH & Co. KG flexen® Exzenterblock Compact
Programme holder Owner of the declaration
IBU – Institut Bauen und Umwelt e.V. Adolf Würth GmbH & Co. KG
Hegelplatz 1 Reinhold-Würth-Str. 12-17
10117 Berlin 74653 Künzelsau
Germany Germany
Declaration number Declared product / declared unit
EPD-AWU-20230267-IBD1-EN flexen® Exzenterblock Compact
This declaration is based on the product category rules: Scope:
Insulating materials made of foam plastics, 01.08.2021 Product line flexen® Exzenterblock Compact Thermal insulation products
(PCR checked and approved by the SVR) for building equipment and industrial insulations made of Polythene-based,
closed-cell foam pipe insulation with a robust protective coating (PEF)
according to EN14313. This declaration
Issue date is an Environmental Product Declaration according to ISO14025 describing
the specific environmental performance of the product produced in
12.09.2023
Belgium at the
site of Eynatten.
The owner of the declaration shall be liable for the underlying information
Valid to
and evidence; the IBU shall not be liable with respect to manufacturer
12.09.2027 information, life cycle assessment data and evidences.
The EPD was created according to the specifications of EN 15804+A2. In
the following, the standard will be simplified as EN 15804.
Verification
The standard EN 15804 serves as the core PCR
Independent verification of the declaration and data according to ISO
14025:2011
internally X externally
Dipl.-Ing. Hans Peters
(Chairman of Institut Bauen und Umwelt e.V.)
Florian Pronold Vito D'Incognito,
(Managing Director Institut Bauen und Umwelt e.V.) (Independent verifier)
1 Environmental Product Declaration - Adolf Würth GmbH & Co. KG - flexen® Exzenterblock Compact
2. Product
consists of around seven basic components. The following
2.1 Product description/Product definition table displays the different elements of formula. This product
flexen® Exzenterblock Compact is the Professional contains substances listed in the candidate list (date:
Polyethylene-based closed-cell foam pipe insulation with a 08.07.2021) exceeding 0.1 percentage by mass: No.
robust PE protective coating, containing recycled PE, for This product contains other carcinogenic, mutagenic, reprotoxic
continuous energy saving and condensation control purposes. (CMR) substances in categories 1A or 1B which are not on the
flexen® Exzenterblock Compact with its rectangular and thin candidate list, exceeding 0.1 percentage by mass: No.
design, it is used in flooring. Biocide products were added to this construction product or it
For the placing on the market of the product in the European has been treated with biocide products (this then concerns a
Union/European Free Trade Association (EU/EFTA) (with the treated product as defined by the (EU) Ordinance on Biocide
exception of Switzerland) - Products No. 528/2012): No.
Thermal Insulation products for building equipment and Name Value Unit
industrial installations cf. PCR. Factory-made polyethylene
LDPE 40.40 %
foam (PEF) and the CE-marking. For the application
Flame retardant 3.2 %
and use, the respective national provisions apply.
LLDPE 2.65 %
2.2 Application Pigment 3.15 %
flexen® Exzenterblock Compact is used to insulate pipes for Internally recycled PE 43.20 %
heating and plumbing.
Volume stabilizer 1.3 %
• Polyethylene foam is a cost-efficient material Blowing Agent 6.10 %
with good insulating properties.
PE and fillers give the aspect of the product. The blowing agent
• Products made of PE foam, containing recycled PE,
causes the expansion during manufacturing. And the flame
yield an excellent
retardants ensure the fire resistance. According the European
cost/performance ratio.
Chemicals Regulation REACH Manufacturers, importers and
• Heat loss control and noise reduction in fresh-and waste
downstream users must register their chemicals and are
water and heating system
responsible for their safe use on their own. For its production
2.3 Technical Data only exclusively verifiably
registered and approved substances are used. flexen®
Constructional data
Exzenterblock Compact does not contain Substances of Very
Performance data of the product in accordance with
High Concern (SVHC). Antimony trioxide and halogenated
the Declaration of Performance with respect to its
flame retardants are applied.
Essential Characteristics according to EN 14313 apply. Further
data:
Name Value Unit 2.6 Manufacture
Gross density 34.3 kg/m3 The manufacturing process consists of a continuous extrusion.
Solid pellets of thermoplastic resin are fed to a melting zone in
Thermal conductivity 0.04 - 0.042 W/(mK)
which the resin is melted, to form a
Reaction To Fire Acc.to EN 13501-1
E flowable thermoplastic mass. The thermoplastic mass is then
depending on the thickness
metered to a mixing zone where the thermoplastic mass is
Max Service Temperature Acc. To EN thoroughly mixed with a blowing agent under pressure. The
100 °C
14707 mixture of thermoplastic resin and blowing agent is then forced
Min Service Temperature 0 °C through a die,
water absorption Acc. to EN 13472 WS005 - which imparts a shape to the thermoplastic mass, into a zone of
lower pressure, such as atmospheric pressure. The blowing
traces quantities of water-soluble ions Cl < 20 – F < 4
- agent expands to form the cells of the foam and the
and pH-value Acc. to EN 13468 - pH 5,8
thermoplastic foam is cooled through an inline water cooler.
The protection coating
2.4 Delivery status
"skin" is applied by co-extrusion. The "skin" is made with solid
The PE products are supplied as tubes. The tubes are pellets of thermoplastic resin and some additives, which is, with
delivered in lengths of 2 m packed in cardboard boxes. The the help of an extruder, applied around the foam. There is not a
insulating sleeves in the flexen® Exzenterblock Compact have foaming agent used in this case. The die is positioned around
a thickness ranging from 9 to 51mm and an inside diameter the
ranging from 15 to 42mm. These products are categorized "naked" foam and deposes a small thickness (± 0.1 mm) of PE
according to thermal conductivity (Lambda*). film on the foam. At the end of this process the profiles are cut
The category of product with lambda 0,040 (W/(mK)) (acc. to at dimension.
EN ISO 8497 and EN 12667) includes flexen® Exzenterblock Quality assurance :
Compact with thickness 9 mm, while the category of product The manufacture is certified ISO 9001 for the quality
with lambda 0,042 (W/(mK)) (acc. to EN12667) includes management. The product corresponds to the product standard
flexen® Exzenterblock Compact with thicknesses from 25 to EN 14313 and has a Declaration of
51mm products. Performance according to the DOP
WÜRTH_LE_0870509015_01_M_flexen_Exzenterblock_Compact
2.5 Base materials/Ancillary materials
(seewww.wuerth.de)
Base materials
2.7 Environment and health during manufacturing
flexen® Exzenterblock Compact is a flexible insulation material
During all manufacturing steps the production follows the
based on Polyethylene with a protecting coating of PE., which
national guidelines and regulations from Belgium. Solar panels
2 Environmental Product Declaration - Adolf Würth GmbH & Co. KG - flexen® Exzenterblock Compact
are installed on the roof of the warehouses. insulation products are still effective after 50 years, it is
assumed that when replacing the piping, the insulation is not
2.8 Product processing/Installation reused and is disposed of with the piping. 50 years is the
flexen® Exzenterblock Compact can be installed using basic minimum Reference Service Life recommended in EN16783.
tools like knives. No special tools, or specific protection is Description of the influences on the ageing of the product when
necessary. When applying adhesives the applied in accordance with the rules of technology.
information given in the relevant safety data sheets is to be
heeded. The recommendations on how to use the product are
described in the application manuals or 2.13 Extraordinary effects
video's. More details are listed on the Web Page WÜRTH Fire
(wuerth.de) Fire
According to flexen® Exzenterblock Compact are classified as
2.9 Packaging EURO CLASS E and therefore have a limited speed of
flexen® Exzenterblock Compact, products are packed in inflammation.
cardboard boxes and transported on reusable pallets. The
Fire protection
packaging material can be recycled. The pallets used to
Name Value
transport the products are taken back or exchanged when the
flexen® Exzenterblock Compact is delivered, so the use of Building material class E
pallets is a close loop economy.
Water
2.10 Condition of use
flexen® Exzenterblock Compact are closed cell foam and
During the use of the product for the purpose for which they are
obtain the better water absorption class WS005 according to
intended, there are no modifications to the product during the
the product standard
use, except if due to extraordinary impact (see point 2.13).
Mechanical destruction
2.11 Environment and health during use
flexen® Exzenterblock Compact are flexible foam covered with
There are no particular aspects of the material composition
a PE protective coating
during the use. flexen® Exzenterblock Compact products are
flexen® Exzenterblock Compact are not UV resistant. The use
used in a wide range and variety of applications for which the
is not recommended for outside applications without
product is intended. The PEF foams fulfil the German, Belgian
complementary UV protection
and French
regulations regarding the emission of VOC with emissions far
2.14 Re-use phase
below the most severe limit values. The Eurofin Product Testing
In principle, if removed carefully, flexen® Exzenterblock
institute, on the demand of
Compact can be reused on any
the CEFEP (European group of PEF and FEF manufacturers)
other piping system of similar dimensions. Any material not
has made a wide range of tests for different PEF products from
suitable for reuse is fully recyclable.
different manufacturers.
The insulation of heating pipes with flexen® Exzenterblock
2.15 Disposal
Compact allows a drastic
flexen® Exzenterblock Compact are fully recyclable using the
reduction of CO emission during the full service life of the
2 same recycling systems as those used for other forms of PE
installation. The quantification of this is not in the topic of this
waste. Any non-recycled material should be disposed of the
EPD, and has to be evaluated in the frame of the LCA from the
materials according to the local regulations, and by the
complete installation
European Waste Catalogue waste code 07 02 13 waste Plastic
"Low Density Polyethylene"
2.12 Reference service life
The function of flexen® Exzenterblock Compact is to ensure the 2.16 Further information
insulation of heating and sanitary installations for a reference Additional information about flexen® Exzenterblock Compact
service life (RSL) of 50
can be found on site WÜRTH (wuerth.de). Here specification
years. This duration is based on the frequency of replacement
clauses, data sheets and application manuals can be found.
of sanitary and heating piping in buildings. Although the
3. LCA: Calculation rules
Name Value Unit
3.1 Declared Unit
Gross density 34.3 kg/m3
The declaration refers to 1 m³ of produced insulation product.
For the LCA calculations, as the product is foam and have Declared unit 1 m3
some tolerances, the density declared is the average between Value for 1 m divided
Conversion factor from 1
the product categories. The thermal conductivity coefficient section of the insulation pipe m
m³ to 1 linear meter
(Lambda-value) and R-value per 25 mm thickness per product ( m²)
brand is provided below as additional information and support Gross Density volume for
for installers. 1 kg 0.02116 m³
Declared unit Thermal Conductivity at
0.040 - 0.042 W/(mK)
40°C
Thermal Conductivity λ: 0.040 W/mK at (40°C)
R-value- thickness: 9 mm: +/- 3,5 (m²K)/W
Thermal Conductivity λ: 0.042 W/mK at (40°C)
R-value- thickness: 25 mm: +/- 3,355 (m²K)/W
depending on the pipe diameter.
3 Environmental Product Declaration - Adolf Würth GmbH & Co. KG - flexen® Exzenterblock Compact
For IBU core EPDs (where clause 3.6 is part of the EPD): for cardboard is a closed cycle with the production process. The
average EPDs, an estimate of the robustness of the LCA flexen® Exzenterblock Compact foam is fully recyclable and
values must be made, e.g. concerning the variability of the can be used as a direct one-for-one substitute for virgin PE-LD
production process, geographical representativeness and the granulates, with only minor additive additions.
influence of background data and preliminary products
compared to the environmental impacts caused by the actual 3.3 Estimates and assumptions
production. The LCA calculation is conducted using the Gabi ts - database.
Not all necessary LCIs are included in the database. Where
data were missing or were unavailable or where suppliers were
3.2 System boundary unable to provide complete information, proxy datasets have
The Data collection refers to the yearly production in 2021 been used.
Module A1 to A3: The environmental burden for the production of pigments, flame
The LCA retardants and volume stabilizers are approximated.
calculation covers the production of the raw materials, transport
of these to 3.4 Cut-off criteria
the plant, the mixing of raw materials according to the Any glue and adhesive tapes used during the installation (A5)
respective recipes, have not been included as
manufacturing of the foam product and packaging for dispatch. quantification of these materials is uncertain and their use by
All production the various installers is too diverse, adhesives and glues are
takes place exclusively in Eynatten, Belgium. not required in all/most cases, but may be used for some
Module A4: applications. In this study no others cut-off criteria have been
The type of transport included in the LCA model is a truck mix applied and all elementary incoming processes as well as all
Euro Cargo 0-6 with diesel fuel. As the product is foam with a energy and water inputs and waste outputs have been counted.
comparatively low density, the product volume is the limiting
factor on loading. flexen® Exzenterblock Compact is rarely 3.5 Background data
the only product loaded in trucks, they are usually grouped with The software system for life cycle engineering GaBi 2021 life
other products of higher density according to the place of cycle database used in the GaBi 10 software environment
destination. trucks has been set to 10% of the mass payload (Service Pack 2021001000) developed by
capacity. Thinkstep AG was used to perform this LCA.
Module A5:
3.6 Data quality
The LCA calculation covers the production of the raw materials,
All the foreground data requiring such energy or raw material
transport of these to
coming from production were verified and cross-checked before
the plant, the mixing of raw materials according to the
being included in the model. Most of the life cycle inventories
respective recipes,
for the basic materials are contained in the GaBi 10 software.
manufacturing of the foam product and packaging for dispatch.
For electrical and thermal energy Belgium-specific grid mixes
All production
and Belgium-specific supply for natural gas were considered.
takes place exclusively in Eynatten, Belgium.
Module B1-B7:
3.7 Period under review
The foam insulation products do not require maintenance,
The production data for the year 2021 were used for the
replacement or refurbishment while in use. The information
realization of this study
modules B1 – B7 are not declared. Although the insulation of
the piping flexen® Exzenterblock Compact contributes to a 3.8 Geographic Representativeness
significant reduction of CO 2 emissions from the heating or Land or region, in which the declared product system is
cooling equipment, this is not taken into account manufactured, used or handled at the end of the product´s
in this LCA. It should, however, be taken into account in the lifespan: Germany
calculation of the environmental impacts of the complete
heating and cooling systems or of the
3.9 Allocation
complete building
Module C1: There is no co-product or by-product generated during the
As for the installation of the product, the disassembly is done production of the products.
manually and does not require any specific equipment. Due to the lack of specific data per production line and product,
Disassembly is generally carried out at the same time as the the energy has been allocated per overall produced volume of
replacement or removal of sanitary pipes. Consequently, there insulation foam.
are no impacts associated with C1. Production waste
Module C2: Most of the production waste from the process (machine start,
Transport at the end-of-life stage is modelled as a Euro Cargo end of production, non-conforming products, etc.) is recycled
0-6 mix truck with diesel fuel. The average distance to either internally in order to be reused in the manufacturing process.
mechanical recycling is assumed to be 100 km. These impacts are accounted for in A1-A3.
Module C3: Installation and End-of-Life waste
The scenario that has been retained for this Life Cycle Installation of the foam products is done by hand and requires
Assessment is the 100% recycling no special equipment apart from a knife. Installation off-cut is
Module C4: not considered in this calculations. Any glue and adhesive
As flexen® Exzenterblock Compact is fully recyclable, the tapes used during the installation phase were not included in
legislation is pushing more in this direction and the overall the LCA
pressure on plastic recycling is growing, therefore the scenario
3.10 Comparability
with 100% recycling is considered.
Basically, a comparison or an evaluation of EPD data is only
Module D:
possible if all the data sets to be compared were created
The end-of-life scenarios for packaging material and product do
according to EN 15804 and the building context, respectively
not deliver any benefits for the next system. The recycling of
the product-specific characteristics of performance, are taken
4 Environmental Product Declaration - Adolf Würth GmbH & Co. KG - flexen® Exzenterblock Compact
into account.
4. LCA: Scenarios and additional technical information
A5 is not declared including the disposal of the packaging
Characteristic product properties of biogenic carbon material on the construction site, the amounts of packaging
The biogenic carbon content quantifies the amount of biogenic materials included in the LCA calculations must be declared as
carbon in a construction product leaving the factory gate, and it technical scenario information for Module A5.
shall be separately declared for the product and for any
accompanying packaging.
If the total mass of biogenic carbon containing materials is less
Transport to the building site (A4)
than 5 % of the total mass of the product and accompanying
packaging, the declaration of biogenic carbon content may be Name Value Unit
omitted. The mass of packaging containing biogenic carbon Litres of fuel 0.069 l/100km
shall always be declared. Transport distance 453 km
Capacity utilisation (including empty runs) 10 %
Note: 1 kg of biogenic carbon is equivalent to 44/12 kg of CO .
2 Gross density of products transported 34.3 kg/m3
Information on describing the biogenic Carbon Content at
In case a reference service life according to applicable ISO
factory gate
standards is declared then the assumptions and in-use
Name ValueUnit
conditions underlying the determined RSL shall be declared. In
kg addition, it shall be stated that the RSL applies to the reference
Biogenic carbon content in product -
C conditions only.
Biogenic carbon content in accompanying kg
5.08
packaging C The same holds for a service life declared by the manufacturer.
Corresponding information related to in-use conditions needs
not be provided if a service life taken from the list of service life
The following technical scenario information is required for the
by BNB is declared.
declared modules and optional for non-declared modules.
Modules for which no information is declared can be deleted;
additional information can also be listed if necessary. Reference service life
Name Value Unit
The following technical information is a basis for the declared Reference service life 50 a
modules or can be used for developing specific scenarios in the
context of a building assessment if modules are not declared End of life (C1-C4)
(MND).
Name Value Unit
Recycling 34.3 kg
5 Environmental Product Declaration - Adolf Würth GmbH & Co. KG - flexen® Exzenterblock Compact
5. LCA: Results
DESCRIPTION OF THE SYSTEM BOUNDARY (X = INCLUDED IN LCA; ND = MODULE OR INDICATOR NOT DECLARED; MNR =
MODULE NOT RELEVANT)
Benefits and
Construction loads beyond
Product stage Use stage End of life stage
process stage the system
boundaries
la ire ta m w a Ry lp p u s tro p s n a rT g n iru tc a fu n a M e h t m o rf tro p s n a rTe tis e h t o t e ta g y lb m e s s A e s U e c n a n e tn ia M ria p e R tn e m e c a lp e R tn e m h s ib ru fe R y g re n e la n o ita re p Oe s u re ta w la n o ita re p Oe s u n o itc u rts n o c -e Dn o itilo m e d tro p s n a rT g n is s e c o rp e ts a W la s o p s iD -e s u e R-y re v o c e R-g n ilc y c e Rla itn e to p
A1 A2 A3 A4 A5 B1 B2 B3 B4 B5 B6 B7 C1 C2 C3 C4 D
X X X X X MND MND MNR MNR MNR MND MND MND X X X X
RESULTS OF THE LCA - ENVIRONMENTAL IMPACT according to EN 15804+A2: 1 m³ flexen® Exzenterblock Compact
Parameter Unit A1-A3 A4 A5 C2 C3 C4 D
GWP-total kg CO 2 eq 9.74E+01 2.72E+00 0 2.86E-01 3.69E+00 0 -8.51E+01
GWP-fossil kg CO 2 eq 9.79E+01 2.73E+00 0 2.87E-01 3.64E+00 0 -8.44E+01
GWP-biogenic kg CO 2 eq -7.84E-01 -3.45E-02 0 -2.81E-03 5.08E-02 0 -7.21E-01
GWP-luluc kg CO 2 eq 2.46E-01 2.44E-02 0 1.94E-03 1.41E-03 0 -1.17E-02
ODP kg CFC11 eq 7.1E-08 3.43E-13 0 2.82E-14 1.51E-10 0 -5.17E-10
AP mol H+ eq 3.52E-01 3.21E-03 0 3.4E-04 5.22E-03 0 -1.17E-01
EP-freshwater kg P eq 5.05E-04 9.64E-06 0 1.03E-06 2.44E-05 0 -1.58E-04
EP-marine kg N eq 5.13E-02 1.09E-03 0 1.13E-04 2.08E-03 0 -3.43E-02
EP-terrestrial mol N eq 5.4E-01 1.29E-02 0 1.35E-03 2.11E-02 0 -3.57E-01
kg NMVOC
POCP 1.96E-01 3.29E-03 0 3.43E-04 5.04E-03 0 -1.12E-01
eq
ADPE kg Sb eq 2.81E-01 1.74E-07 0 2.89E-08 2.12E-06 0 -2.15E-05
ADPF MJ 3E+03 3.59E+01 0 3.77E+00 1.09E+02 0 -3.25E+03
m3 world eq
WDP 6.83E+00 3.19E-02 0 3.21E-03 2.63E-01 0 -1.44E+00
deprived
GWP = Global warming potential; ODP = Depletion potential of the stratospheric ozone layer; AP = Acidification potential of land and water; EP =
Eutrophication potential; POCP = Formation potential of tropospheric ozone photochemical oxidants; ADPE = Abiotic depletion potential for non-fossil
resources; ADPF = Abiotic depletion potential for fossil resources; WDP = Water (user) deprivation potential)
RESULTS OF THE LCA - INDICATORS TO DESCRIBE RESOURCE USE according to EN 15804+A2: 1 m³ flexen® Exzenterblock
Compact
Parameter Unit A1-A3 A4 A5 C2 C3 C4 D
PERE MJ 4.94E+02 2.61E+00 0 2.61E-01 6.74E+01 0 -2.44E+02
PERM MJ 0 ND ND ND ND ND ND
PERT MJ 4.94E+02 2.61E+00 0 2.61E-01 6.74E+01 0 -2.44E+02
PENRE MJ 1.2E+03 3.61E+01 0 3.79E+00 1.09E+02 0 -3.26E+03
PENRM MJ 1.82E+03 ND ND ND ND ND ND
PENRT MJ 3.02E+03 3.61E+01 0 3.79E+00 1.09E+02 0 -3.26E+03
SM kg 1.26E+01 ND ND ND ND ND ND
RSF MJ 0 ND ND ND ND ND ND
NRSF MJ 0 ND ND ND ND ND ND
FW m3 5.48E-01 2.86E-03 0 3.02E-04 3.09E-02 0 -3.85E-01
PERE = Use of renewable primary energy excluding renewable primary energy resources used as raw materials; PERM = Use of renewable primary
energy resources used as raw materials; PERT = Total use of renewable primary energy resources; PENRE = Use of non-renewable primary energy
excluding non-renewable primary energy resources used as raw materials; PENRM = Use of non-renewable primary energy resources used as raw
materials; PENRT = Total use of non-renewable primary energy resources; SM = Use of secondary material; RSF = Use of renewable secondary fuels;
NRSF = Use of non-renewable secondary fuels; FW = Use of net fresh water
RESULTS OF THE LCA – WASTE CATEGORIES AND OUTPUT FLOWS according to EN 15804+A2:
1 m³ flexen® Exzenterblock Compact
Parameter Unit A1-A3 A4 A5 C2 C3 C4 D
HWD kg 7.83E-04 1.12E-10 0 2E-11 1.16E-08 0 -3.04E-07
NHWD kg 4.03E+00 5.5E-03 0 6.17E-04 1.45E-01 0 -8.99E-01
RWD kg 1.3E-01 6.75E-05 0 7.03E-06 2.54E-02 0 -2.72E-02
CRU kg ND ND ND ND ND ND ND
MFR kg ND ND 1.26E+01 ND 4.73E+01 ND ND
MER kg ND ND ND ND ND ND ND
EEE MJ ND ND ND ND ND ND ND
EET MJ ND ND ND ND ND ND ND
6 Environmental Product Declaration - Adolf Würth GmbH & Co. KG - flexen® Exzenterblock Compact
HWD = Hazardous waste disposed; NHWD = Non-hazardous waste disposed; RWD = Radioactive waste disposed; CRU = Components for re-use;
MFR = Materials for recycling; MER = Materials for energy recovery; EEE = Exported electrical energy; EET = Exported thermal energy
RESULTS OF THE LCA – additional impact categories according to EN 15804+A2-optional:
1 m³ flexen® Exzenterblock Compact
Parameter Unit A1-A3 A4 A5 C2 C3 C4 D
Disease
PM 1.72E-05 2.42E-08 0 2.6E-09 4.16E-08 0 -8.81E-07
incidence
IR kBq U235 eq 1.09E+01 1.01E-02 0 1.06E-03 1.77E+00 0 -2.69E+00
ETP-fw CTUe 1.64E+03 2.55E+01 0 2.67E+00 4.25E+01 0 -1.55E+03
HTP-c CTUh 4.27E-08 5.22E-10 0 5.51E-11 1.05E-09 0 -3.81E-08
HTP-nc CTUh 3.34E-06 2.8E-08 0 3.02E-09 3.25E-08 0 -1.77E-06
SQP SQP 3.01E+02 1.5E+01 0 1.6E+00 6.87E+01 0 -1.66E+02
PM = Potential incidence of disease due to PM emissions; IR = Potential Human exposure efficiency relative to U235; ETP-fw = Potential comparative
Toxic Unit for ecosystems; HTP-c = Potential comparative Toxic Unit for humans (cancerogenic); HTP-nc = Potential comparative Toxic Unit for humans
(not cancerogenic); SQP = Potential soil quality index
Disclaimer 1 – for the indicator “Potential Human exposure efficiency relative to U235”.This impact category deals mainly with the
eventual impact of low dose ionizing radiation on human health of the nuclear fuel cycle. It does not consider effects due to possible
nuclear accidents, occupational exposure or radioactive waste disposal in underground facilities. Potential ionizing radiation from the
soil, radon and from some construction materials is also not measured by this indicator.
Disclaimer 2 – for the indicators “abiotic depletion potential for non-fossil resources”, “abiotic depletion potential for fossil resources”,
“water (user) deprivation potential, deprivation-weighted water consumption”, “potential comparative toxic unit for ecosystems”,
“potential comparative toxic unit for humans – cancerogenic”, “Potential comparative toxic unit for humans - not cancerogenic”,
“potential soil quality index”. The results of this environmental impact indicator shall be used with care as theuncertainties on these
results are high as there is limited experience with the indicator. This EPD was created using a software tool.
6. LCA: Interpretation
The use of internal recycled material in flexen® Exzenterblock recyclable; the choice for the end of life was that of 100%
Compact reduces the need for raw materials and avoids recycling. This avoids the use of new raw materials and or the
wasting resources. flexen® Exzenterblock Compact has a very exploitation of
low density, which means that little raw material is needed for renewable or non-renewable resources. The end of life in 100%
high insulation landfill has a
efficiency, which results in significant energy savings. In slight impact, especially from the point of view of climate
addition, flexen® Exzenterblock Compact is largely made of change. However,
the 100% incineration scenario has the greatest impact
low-density polyethylene, so it is fully recyclable and can be
because during incineration there is a significant release of
recycled when it reaches the end of its life. As there is a
variation in density between the different references of the carbon dioxide. The insulation with flexen® Exzenterblock
flexen® Exzenterblock Compact range, a sensitivity Compact of the sanitary and heating piping contributes to a
significant reduction of CO emissions from the heating or
analysis has been performed. The results of the LCA are given 2
for 1m3 of product calculated with an average weighted foam cooling equipment, this is not considered in this LCA. It should,
density of 34,4 kg/m³. For the lowest density, the impacts are however, be taken into account in the calculation of
lowered by 12,4 % and for the highest density the impacts environmental impacts of the complete heating and cooling
should be majored by 10,9 %. Most references are very close systems or of the complete building. One way to continue to
to the average density, reduce the environmental impact of
but all impact factors can be recalculated based on the the flexen® Exzenterblock Compact would be to continue to
product's density. When diversify our energy
we analyse the complete life cycle, we see that the most sources by switching more and more to renewable energies. To
impacting part for all this end, after
environmental impact factors is the production module and having greatly increased the number of photovoltaic panels, the
more particularly the production plant will acquire a cogeneration system. Looking for
raw materials part. With regard to global warming for the more eco-responsible suppliers must also be
complete life cycle, more than 94% comes from the production put in place, as well as finding raw materials manufactured
module 1,6% from transport to the places of installation and locally to avoid
3,9% comes from the end of life. A more in-depth analysis of long-distance transport as much as possible. An analysis of the
the plant's carbon
production module A1 to A3 shows that the production of raw footprint, which is currently being carried out, should enable to
materials and their identify
transport account for almost 95% of the impact Global Warming areas for improvement and find solutions to achieve the goal of
Potential. As the flexen® Exzenterblock Compact is fully zero carbon.
7. Requisite evidence
7.1. VOC emissions (determined after
Eurofins Product Testing A/S has tested a wide range and consideration of the real-life applications of PEF products (in
variety of typical PEF (Polyethylene foam) products marketed in living rooms) and recommendations by the experts of the test
the EU from CEFEP (European Group of PEF/FEF institute) all results were found to be
manufacturers) Based on the loading factor 0.05m²/m3 clearly below the limit values. For all samples below 100mg/m3
7 Environmental Product Declaration - Adolf Würth GmbH & Co. KG - flexen® Exzenterblock Compact
TVOC after 28 days. Certificates are available on request. 7.1
VOC emissions 7.2 Leaching
For products used in indoor applications. According to EN 13468 the content of water-soluble chloride
Test procedure to AgBB diagram indicating the measuring ions for flexen® Exzenterblock Compact is <20mg/kg
agency, date and results as a range of values. At least the
following must be declared:
8. References
EN 1602 CEN/TR 15941
EN 1602: 2013: Thermal insulating products for CEN/TR 15941: Sustainability of construction works -
building applications - Determination of the apparent Environmental product declarations - Methodology for
density selection and use of generic data
EN ISO 8497 CEN TS 16516
EN ISO 8497: Thermal insulation - Determination of CEN TS 16516: AgBB, ISO 16000-3, /ISO 16000-6/,
steady-state thermal transmission properties of thermal /ISO16000-9/, /ISO 16000-11/ Construction products -
insulation for circular pipes Assessment of release of dangerous substances.
Determination of emissions into indoor air
ISO 9001
ISO 9001: 2015: Quality management systems. EN 16783: 2017
EN 16783: 2017 Thermal insulation products - Product
EN13472 category rules (PCR) for factory made and in-situ
EN 13472: Thermal insulating products for building equipment formed products for preparing environmental product
and declarations.
industrial installations - Determination of short term water
absorption by Candidate List Substances of Very High Concern
partial immersion of preformed pipe insulation SVCH: date: 08.07.2021) exceeding 0.1 percentage by mass
EN 13468 CEFEP
EN 13468: Thermal insulating products for building equipment CEFEP: European group of PEF and FEF manufacturers
and
industrial installations - Determination of trace quantities of Eurostat
water-soluble European Statistics: Recovery rates for packaging
chloride, fluoride, silicate, and sodium ions and pH waste Paper and cardboard packaging for the
European Union 27 countries 2014
EN 13501-1 http://ec.europa.eu/eurostat/home
EN 13501-1:2007+A1: 2013 Fire classification of
construction products and building elements - Eurofins
Classification using test data from reaction to fire tests Eurofins: Eurofins Scientific is a group of international life
sciences
ISO 14001 companies which provide a unique range of analytical testing
ISO 14001: 2015 Environmental management services to
systems. clients across multiple industries, http://www.eurofins.com
EN ISO 14025 Gabi ts
EN ISO 14025: 2011-10: Environmental labels and GaBi 10 GaBi Software-System and Database for Life
declarations — Type III environmental declarations — Cycle Engineering Copyright © 1992-2021 Sphera
Principles and procedures Solutions Gmbh Version: 10.5.0.78 DB Schema 8007
ISO 14040 Institut Bauen und Umwelt
ISO 14040: Environmental management — Life cycle Institut Bauen und Umwelt e.V., Berlin(pub.): General
assessment — Principles and framework Instructions for the EPD Programme of Institut Bauen
und Umwelt e.V., Version 2.0 2021.
ISO 14044
ISO 14044: Environmental management — Life cycle Product Category Rules for Building-Related
assessment — Requirements and guidelines Products and Services
Institute Construction and Environment e.V. (IBU)
EN 14707 Part A: Calculation Rules for the Life Cycle
EN 14707: 2012: Thermal insulating products for Assessment and Requirements on the Project Report
building equipment and industrial installations. Version 1.7
Determination of maximum service temperature for
preformed pipe insulation PCR Guidance-Texts for Building-Related Products
and Services
EN 15804 From the range of Environmental Product Declarations
EN 15804: 2012-04 + A1 2014: Sustainability of of Institute Construction and Environment e.V. (IBU)
construction works — Environmental Product Part B: Requirements on the EPD for Insulating
Declarations — Core rules for the product category of materials made of foam plastics
construction products Version 1.6 (Template) Version 1.2 (PCR specific)
8 Environmental Product Declaration - Adolf Würth GmbH & Co. KG - flexen® Exzenterblock Compact
REACH Sphera Solutions Gmbh. GaBi 10 LCI documentation.
According the European Chemicals Regulation REACH GaBi Databases (sphera.com) Stuttgart
manufacturers, The literature referred to in the Environmental Product
importers and downstream users must register their chemicals Declaration must be listed in full.Standards already fully quoted
and are in the EPD do not need to be listed here again.
responsible for their safe use. The current version of PCR Part A and PCR Part B of the PCR
document on which they are based must be referenced.
Sphera
9 Environmental Product Declaration - Adolf Würth GmbH & Co. KG - flexen® Exzenterblock Compact
Publisher
Institut Bauen und Umwelt e.V. +49 (0)30 3087748- 0
Hegelplatz 1 info@ibu-epd.com
10117 Berlin www.ibu-epd.com
Germany
Programme holder
Institut Bauen und Umwelt e.V. +49 (0)30 3087748- 0
Hegelplatz 1 info@ibu-epd.com
10117 Berlin www.ibu-epd.com
Germany
Author of the Life Cycle Assessment
Owner of the Declaration
Adolf Würth GmbH & Co. KG +49 7940/15-0
Reinhold-Würth-Str. 12-17 info@wuerth.com
74653 Künzelsau www.wuerth.de
Germany
10 Environmental Product Declaration - Adolf Würth GmbH & Co. KG - flexen® Exzenterblock Compact
