ENVIRONMENTAL PRODUCT DECLARATION
as per ISO 14025 and EN 15804+A2
Owner of the Declaration JSW Steel Italy Piombino
Publisher Institut Bauen und Umwelt e.V. (IBU)
Programme holder Institut Bauen und Umwelt e.V. (IBU)
Declaration number EPD-JSW-20240097-IBA1-EN
Issue date 18.04.2024
Valid to 17.04.2029
JSW steel rail
JSW Steel Italy Piombino S.p.A.
www.ibu-epd.com | https://epd-online.com
1. General Information
JSW Steel Italy Piombino S.p.A. JSW steel rail
Programme holder Owner of the declaration
IBU – Institut Bauen und Umwelt e.V. JSW Steel Italy Piombino
Hegelplatz 1 Largo Caduti sul Lavoro 21
10117 Berlin 57025 Piombino
Germany Italy
Declaration number Declared product / declared unit
EPD-JSW-20240097-IBA1-EN 1 ton of steel rail
This declaration is based on the product category rules: Scope:
Rails forming a track for vehicles, 01.08.2021 The EPD declaration refers to 1 tonne of rail product manufactured at the
(PCR checked and approved by the SVR) JSW Steel Italy plant in Piombino (Italy).
The data used is based on one year's manufacturing of product 60 E1.
This product has been identified as representative of JSW Steel Italy's total
Issue date production for the year 2022 which also includes the following products:
50E5, 60E2, 54E2, 54E1, 60E1A2 and 115RE2010
18.04.2024
For this EPD, LCA model created by the bloom supplier (JSW Steel
Limited) in order to realise the EPD Average of Finished Long Products
(Steel) was used for the bloom production phase.
Valid to
17.04.2029 The owner of the declaration shall be liable for the underlying information
and evidence; the IBU shall not be liable with respect to manufacturer
information, life cycle assessment data and evidences.
The EPD was created according to the specifications of EN 15804+A2. In
the following, the standard will be simplified as EN 15804.
Verification
The standard EN 15804 serves as the core PCR
Independent verification of the declaration and data according to ISO
14025:2011
Dipl.-Ing. Hans Peters internally X externally
(Chairman of Institut Bauen und Umwelt e.V.)
Florian Pronold Vito D'Incognito,
(Managing Director Institut Bauen und Umwelt e.V.) (Independent verifier)
1 Environmental Product Declaration - JSW Steel Italy Piombino S.p.A. - JSW steel rail
2. Product
2.1 Product description/Product definition 2.5 Base materials/Ancillary materials
In the railway sector, JSW Steel Italy Piombino manufactures The starting material for rail production in Piombino consists of
rails, switch and crossing rails and check rails at its Piombino 100 % casting blooms of square and rectangular cross-
plant, in different grades and sections according to the main sections. Chemical composition is in accordance with the
international and European standards or according to customer standards indicated in chapter 2.3.
specifications, in lengths between 4 and 108 m. The
• This product contains substances listed in the candidate
manufacturing of joints is not included in this study.
list exceeding 0.1 percentage by mass: NO
For the placing on the market in the European Union/European
Free Trade Association (EU/EFTA) (with the exception of • This product/article/at least one partial article contains
Switzerland) the following legal provisions apply: other carcinogenic, utagenic, reprotoxic ( CMR)
substances in categories 1A or 1B which are not on the
• Directive (EU) 2016/797 of the European Parliament
candidate list, exceeding 0.1 percentage by mass: NO'
and of the Council of 11 May 2016 on the interoperability
of the rail system within the European Union • Biocide products were added to this construction
• Commission regulation 1299/2014 of 18th November product or it has been treated with biocide products (this
2014 concerning a technical specification for then concerns a treated product as defined by the (EU)
interoperability relating to the infrastructure subsystem Ordinance on Biocide Products No. 528/2012): NO
of the rail system in the European Union,
2.6 Manufacture
• Commission Implementing Regulations (EU) 2019/776
The source material for the production of rails at Piombino are
and (EU) 2020/387
long semi-finished products of square and rectangular cross-
For the use and application of the product the respective
sections that the site supplies from JSW group steel mills. The
national provisions at the place of use, apply.
blooms are produced with ore coming from proprietary mines.
2.2 Application The production cycle uses only internally sourced scrap and
In the railway sector, JSW Steel Italy Piombino products are involves degassing and continuous casting. For more
mainly for use in: information regarding bloom production, please refer to the
EPD Average of Finished Long Products (Steel) by JSW Steel
• High-speed lines
Limited.
• Mixed railway lines (passenger and freight)
Blooms arrive in Piombino by ship and are transported to the
• Urban public transport (subways and trams)
rolling plant for subsequent use as feed in the production of
• Railways switches
rails. The rolling mill is equipped with a walking beam furnace, a
roughing stand, two reversible stands, a finishing stand and a
2.3 Technical Data
still-air cooling plate. The standard length produced is 108m.
The technical specifications of the products within the scope of
Long rails, previously straightened and subjected to quality
the EPD are reported in the following main standards:
controls (NDT checks: eddy current, US and visual testing), are
• EN 13674 – 1 then transported by internal rail link to the Service Centre (CSE)
• EN 13674 – 2 for cutting to size and possible drilling according to customer
• EN 13674 – 3 specifications, before being placed in the warehouse and
• EN 13674 – 4 subsequent shipment.
• UIC 860.O
• BS 11 2.7 Environment and health during manufacturing
• AREMA Piombino plant is certified in accordance with the following
• Customer specifications standards:
Constructional data for representative product • ISO 9001
Name Value Unit • ISO 14001
• ISO 45001
Density 7850 kg/m3
• ISO 50001
Tensile strength > 880 N/mm2 and performs periodic internal and third-party audits to ensure
Grade of material according to the delivery compliance with its Management System procedures.
R260 -
standards A monitoring and control plan is applied to verify compliance
Hardness > 260 HBV with the level of emissions required by current regulations.
The company promotes an approach based on minimizing
Elongation > 10 %
consumption and environmental impacts by applying the PDCA
11.5 -
Lineal Thermal Expansion Coefficient (LTEC) 10-6ºC method.
12.0
2.8 Product processing/Installation
Performance data of the product with respect to its
characteristics are in accordance with the relevant technical Rails produced in Piombino are usually processed directly by
provision (no CE-marking). customers at the installation site.
2.4 Delivery status 2.9 Packaging
JSW Steel Italy Piombino rails are supplied in as-rolled The rails are usually supplied loose and secured for transport
conditions, in the following linear weight range: by means of cranes equipped with a dedicated gripping device
called 'Rail Grip'. Contact damage is avoided by the use of
• rails: 27 - 70 kg/m
spacing timber.
• tongue bars: 50 - 70 kg/m
Rails can be cut according to customer requirements. Max 2.10 Condition of use
supplied length: 108m
2 Environmental Product Declaration - JSW Steel Italy Piombino S.p.A. - JSW steel rail
The composition of the rails does not change during the life
cycle. Mechanical destruction
Inspection and maintenance operations of rails in use are No environmental impact is expected due to unforeseeable
carried out by customers in accordance with their experience mechanical destruction.
and relevant international Standards.
2.14 Re-use phase
2.11 Environment and health during use Rails are 100 % steel, which is totally recyclable as a raw
No health or environmental impacts are recorded during the life material in the steelmaking process. In fact, steel undergoes no
cycle of the rails. degradation during the production cycle and can therefore be
recycled countless times.
2.12 Reference service life
This EPD does not cover modules B1-B7. A reference service 2.15 Disposal
life for rails is not declared. The declared product can be entirely recycled as an EoW or
waste. The waste Code in accordance with the European
2.13 Extraordinary effects Waste Catalogue (EWC) is 17 04 05.
Fire
Rails aren't flammable without the release of flammable gasses 2.16 Further information
or fumes during use. Other information about the declared product are available on
Water the JSW Steel Italy Piombino website at
No environmental impact is expected due to the unforeseeable https://www.jswitaly.com/
influence of water, e.g. flooding.
3. LCA: Calculation rules
3.1 Declared Unit Module C2| Transport to the processing/disposal site
This environmental product declaration refers to a declared unit After the dismantling, the rail is transported to the end-of-life
of 1 ton of representative JSW Steel Italy rail in accordance processing where all the impacts related to the transport
with the PCR "Rails forming a track for vehicles", 01/08/2021. processes are considered.
The declaration type is according to EN 15804+A2: Cradle to
gate (A1-A3) with modules C1–C4 and module D. Module C3| Waste processing
Declared unit and mass reference Product flows that reach Module D for recycling leave the
product system in C3.
Name Value Unit
Declared unit 1 t
Module C4| Disposal
Density 7850 kg/m3 There is no disposal (C4) as the considered End-of-Life
scenario is 100 % recycling.
Other declared units are allowed if the conversion is shown
transparently.
Module D| Benefits and loads beyond the system
boundaries
This EPD covers all types of rails produced by JSW Steel Italy
The potential for substituting primary steel with a recycling
in 2022. The calculation were performed based on the
scenario (100 % of the product) is set forth in Module D. The
manufacturing data of the 60E1 rails which were identified as
100 % recycling scenario is based on the fact that the product
representative for the whole production, since they account for
still retains an important economic value at its end of life, so
83 % of 2022 annual production.The products covered by this
that it can be sold externally.
EPD are: 60E1 (grade R260), 50E5 (grade R260), 60E2 (grade
R260), 54E2 (grade R260), 54E1 (grade R260/R260Mn),
3.3 Estimates and assumptions
60E1A2 and 115R2010 (grade Arema low Alloy).
The blooms under consideration come from 2 separate plants:
The representativeness of the data considered for all JSW
Steel Italy products was analysed by means of a sensitivity • JSW Steels, Salem, Tamil Nadu (plant on which the
analysis. EPD Average of Finished Long Products (Steel) is
based)
3.2 System boundary • JSW Steel Limited, Raigarh Works (Formerly known as
This life cycle assessment refers to a cradle-to-gate analysis Monnet Ispat&Energy LtD), Naharpali, Dist Raigarh,
with options. The following life cycle phases are taken into Chhattishgarh
consideration in the analysis: For the production of virgin material in A1, only the data
provided by the supplier was used, assuming that the
Module A1-A3| Product stage production impact of the JSW Steel Limited, Raigarh Works
The product stage includes provision of all materials, products, (corresponding to 1 % of the blooms supplied to JSW Italy) was
auxiliaries and energy, as well as waste processing up to the the same as that of JSW Steels, Salem, Tamil Nadu
end-of-waste state or disposal of final residues during the (corresponding to 99 % of the blooms supplied to JSW Italy).
product stage. All assumptions are explained through detailed documentation
These modules consider the manufacturing of raw materials in and correspond to the best possible representation of reality on
particular steel bloom, the transport to the production site and the basis of the available data.
the production processes of the product under study.
3.4 Cut-off criteria
Module C1 | Dismantling No cut-offs were applied in the study.
The rail dismantling takes place in the C1 module which
3.5 Background data
considers energy production and consumption in terms of
Data from the Managed LCA Content (GaBi database 2023.2)
diesel and all the emissions connected with the fuel-burning
was used as background data.
process.
3 Environmental Product Declaration - JSW Steel Italy Piombino S.p.A. - JSW steel rail
lifespan: Global
3.6 Data quality
The foreground data collected at JSW Steel Italy Piombino are
based on the volumes consumed and produced annually. All 3.9 Allocation
primary data refers to rail manufacturing were collected by JSW The data collected for 2022 rails production was allocated by
Steel Italy Piombino and refer to the production year 2022. mass on the production of 60E1 rails. To understand the
In selecting the background data, the technological, allocations made by the bloom producer who provided the
geographical and temporal representativeness of the database primary data (JSW steel limited), please refer to the EPD
was analysed. In the absence of specific data, generic datasets Average of Finished Long Products (Steel).
or representative average data were used. During the LCA modelling, no allocations were performed.
The overall quality of the data is considered good. Information about the allocation procedure of single datasets is
In order to assess the representativeness of this EPD for all documented in https://sphera.com/product-sustainability-gabi-
rails produced by JSW Steel Italy Piombino, an analysis of data-search/.
variance was carried out, which showed a minimal variation in
3.10 Comparability
results between the different products.
Basically, a comparison or an evaluation of EPD data is only
possible if all the data sets to be compared were created
3.7 Period under review according to EN 15804 and the building context, respectively
Foreground data were collected in the 2022 production year. the product-specific characteristics of performance, are taken
into account. The Managed LCA Content (GaBi database
3.8 Geographic Representativeness 2023.2) has been used.
Land or region, in which the declared product system is
manufactured, used or handled at the end of the product´s
4. LCA: Scenarios and additional technical information
Characteristic product properties of biogenic carbon
No biogenic carbon is contained in the product concerned.
End of life (C1 - C4)
According to EN 15804+A2 it is requested to declare 100 %
Note: 1 kg of biogenic carbon is equivalent to 44/12 kg of CO2.
End-of-Life scenarios (here considered: 100 % recycling).
Name Value Unit
Information on describing the biogenic carbon content at Collected waste 1000 kg
factory gate Recycling 1000 kg
Name ValueUnit
Reuse, recovery and/or recycling potentials (D), relevant
Biogenic carbon content in product - kg scenario information
C
Name Value Unit
Biogenic carbon content in accompanying kg
- Net flow of steel scrap 1000 kg
packaging C
4 Environmental Product Declaration - JSW Steel Italy Piombino S.p.A. - JSW steel rail
5. LCA: Results
DESCRIPTION OF THE SYSTEM BOUNDARY (X = INCLUDED IN LCA; MND = MODULE OR INDICATOR NOT DECLARED; MNR
= MODULE NOT RELEVANT)
Benefits and
Construction loads beyond
Product stage Use stage End of life stage
process stage the system
boundaries
la ire ta m w a Ry lp p u s tro p s n a rT g n iru tc a fu n a M e h t m o rf tro p s n a rTe tis e h t o t e ta g y lb m e s s A e s U e c n a n e tn ia M ria p e R tn e m e c a lp e R tn e m h s ib ru fe R y g re n e la n o ita re p Oe s u re ta w la n o ita re p Oe s u n o itc u rts n o c -e Dn o itilo m e d tro p s n a rT g n is s e c o rp e ts a W la s o p s iD -e s u e R-y re v o c e R-g n ilc y c e Rla itn e to p
A1 A2 A3 A4 A5 B1 B2 B3 B4 B5 B6 B7 C1 C2 C3 C4 D
X X X MND MND MND MND MNR MNR MNR MND MND X X X X X
RESULTS OF THE LCA - ENVIRONMENTAL IMPACT according to EN 15804+A2: 1 t of steel rail
Parameter Unit A1 A2 A3 C1 C2 C3 C4 D
GWP-total kg CO 2 eq 2.7E+03 1.52E+02 1.27E+02 6.38E-01 1.16E+01 0 0 -2.1E+03
GWP-fossil kg CO 2 eq 2.7E+03 1.5E+02 1.27E+02 6.1E-01 1.11E+01 0 0 -2.1E+03
GWP-biogenic kg CO 2 eq 3.38E-01 1.73E+00 2.29E-01 2.79E-02 5.04E-01 0 0 1.27E+00
GWP-luluc kg CO 2 eq 5.15E-01 2.15E-03 1.79E-02 6.14E-05 1.13E-03 0 0 -7.63E-01
ODP kg CFC11 eq 5.81E-06 3.25E-12 4.59E-11 6.83E-14 1.26E-12 0 0 2.62E-09
AP mol H+ eq 2.61E+01 2.51E+00 6.06E-02 3.06E-03 5.69E-02 0 0 -3.55E+00
EP-freshwater kg P eq 3.41E-04 2.32E-05 9.32E-05 1.48E-07 2.73E-06 0 0 -7.35E-04
EP-marine kg N eq 4.2E+00 1.06E+00 1.21E-01 1.45E-03 2.77E-02 0 0 -8.64E-01
EP-terrestrial mol N eq 4.6E+01 1.17E+01 3.07E-01 1.59E-02 3.05E-01 0 0 -9.3E+00
kg NMVOC
POCP 1.22E+01 2.8E+00 7.38E-02 4.1E-03 5.49E-02 0 0 -2.92E+00
eq
ADPE kg Sb eq 1.9E-05 7.81E-07 3.39E-05 8E-09 1.48E-07 0 0 -3.57E-05
ADPF MJ 3.81E+04 2E+03 1.07E+02 8.74E+00 1.61E+02 0 0 -1.36E+04
m3 world eq
WDP 9.37E+01 1.92E-01 6.92E+01 1.5E-03 2.77E-02 0 0 -7.75E+01
deprived
GWP = Global warming potential; ODP = Depletion potential of the stratospheric ozone layer; AP = Acidification potential of land and water; EP =
Eutrophication potential; POCP = Formation potential of tropospheric ozone photochemical oxidants; ADPE = Abiotic depletion potential for non-fossil
resources; ADPF = Abiotic depletion potential for fossil resources; WDP = Water (user) deprivation potential)
RESULTS OF THE LCA - INDICATORS TO DESCRIBE RESOURCE USE according to EN 15804+A2: 1 t of steel rail
Parameter Unit A1 A2 A3 C1 C2 C3 C4 D
PERE MJ 1.14E+03 2.7E+00 2.77E+01 5.82E-02 1.07E+00 0 0 1.51E+03
PERM MJ 0 0 0 0 0 0 0 0
PERT MJ 1.14E+03 2.7E+00 2.77E+01 5.82E-02 1.07E+00 0 0 1.51E+03
PENRE MJ 3.81E+04 2E+03 1.07E+02 8.79E+00 1.62E+02 0 0 -1.37E+04
PENRM MJ 0 0 0 0 0 0 0 0
PENRT MJ 3.81E+04 2E+03 1.07E+02 8.79E+00 1.62E+02 0 0 -1.37E+04
SM kg 0 0 0 0 0 0 0 1E+03
RSF MJ 2.97E-06 0 0 0 0 0 0 0
NRSF MJ 4.51E-05 0 0 0 0 0 0 0
FW m3 2.5E+00 6.32E-03 1.56E+00 8.16E-05 1.51E-03 0 0 -5.36E-01
PERE = Use of renewable primary energy excluding renewable primary energy resources used as raw materials; PERM = Use of renewable primary
energy resources used as raw materials; PERT = Total use of renewable primary energy resources; PENRE = Use of non-renewable primary energy
excluding non-renewable primary energy resources used as raw materials; PENRM = Use of non-renewable primary energy resources used as raw
materials; PENRT = Total use of non-renewable primary energy resources; SM = Use of secondary material; RSF = Use of renewable secondary fuels;
NRSF = Use of non-renewable secondary fuels; FW = Use of net fresh water
RESULTS OF THE LCA – WASTE CATEGORIES AND OUTPUT FLOWS according to EN 15804+A2:
1 t of steel rail
Parameter Unit A1 A2 A3 C1 C2 C3 C4 D
HWD kg 1.66E-05 7.62E-11 2.94E-07 1.5E-11 2.76E-10 0 0 1.31E-07
NHWD kg 1.83E+01 2.93E-02 1.11E+00 8.14E-04 1.5E-02 0 0 -3.4E+01
RWD kg 1.54E-01 2.65E-04 2.21E-03 1.4E-05 2.58E-04 0 0 4.8E-01
CRU kg 0 0 0 0 0 0 0 0
MFR kg 0 0 3.26E+01 0 0 0 0 1E+03
MER kg 0 0 0 0 0 0 0 0
EEE MJ 0 0 0 0 0 0 0 0
EET MJ 0 0 0 0 0 0 0 0
HWD = Hazardous waste disposed; NHWD = Non-hazardous waste disposed; RWD = Radioactive waste disposed; CRU = Components for re-use;
MFR = Materials for recycling; MER = Materials for energy recovery; EEE = Exported electrical energy; EET = Exported thermal energy
5 Environmental Product Declaration - JSW Steel Italy Piombino S.p.A. - JSW steel rail
RESULTS OF THE LCA – additional impact categories according to EN 15804+A2-optional:
1 t of steel rail
Parameter Unit A1 A2 A3 C1 C2 C3 C4 D
Disease
PM ND ND ND ND ND ND ND ND
incidence
IR kBq U235 eq ND ND ND ND ND ND ND ND
ETP-fw CTUe ND ND ND ND ND ND ND ND
HTP-c CTUh ND ND ND ND ND ND ND ND
HTP-nc CTUh ND ND ND ND ND ND ND ND
SQP SQP ND ND ND ND ND ND ND ND
PM = Potential incidence of disease due to PM emissions; IR = Potential Human exposure efficiency relative to U235; ETP-fw = Potential comparative
Toxic Unit for ecosystems; HTP-c = Potential comparative Toxic Unit for humans (cancerogenic); HTP-nc = Potential comparative Toxic Unit for humans
(not cancerogenic); SQP = Potential soil quality index
Disclaimer 1 – for the indicator “Potential Human exposure efficiency relative to U235”. This impact category deals mainly with the
eventual impact of low-dose ionizing radiation on human health of the nuclear fuel cycle. It does not consider effects due to possible
nuclear accidents, occupational exposure or radioactive waste disposal in underground facilities. Potential ionizing radiation from the
soil, radon and from some construction materials is also not measured by this indicator.
Disclaimer 2 – for the indicators “abiotic depletion potential for non-fossil resources”, “abiotic depletion potential for fossil resources”,
“water (user) deprivation potential, deprivation-weighted water consumption”, “potential comparative toxic unit for ecosystems”,
“potential comparative toxic unit for humans – cancerogenic”, “Potential comparative toxic unit for humans - not cancerogenic”,
“potential soil quality index”. The results of this environmental impact indicator shall be used with care as the uncertainties on these
results are high as there is limited experience with the indicator.
6. LCA: Interpretation
The major contributor to all impact categories is steel indicator and 38 % of WDP) and energy consumption, including
production (module A1), accounting for more than 55 % of the both electricity and natural gas production (15 % of EP-
impacts in each category. Module A1 alone contributes to 90 % freshwater indicator and 6 % of WDP).
of Global Warming Potential (GWP) indicator, while the whole End-of-life modules have negligible impacts in almost all
upstream phase (A1-A2) generates almost the entire impact (95 categories; the main contribution is derived from waste
%). Energy is the second contributor to GWP, accounting for transportation (Module C2). Conversely, Module D has a
almost 8 % of the total, mainly due to the natural gas used considerable value when compared to the other indicators. In
during rail production. Module A2 has a relative impact on fact, for total GWP and EP freshwater, the credits from the steel
marine and terrestrial eutrophication indicators and for the recycling process reach more than -30 % in terms of relative
POCP, while module A3 (manufacturing) impacts mainly impacts. Not in all indicators, however, is a credit associated
freshwater eutrophication indicators and the WDP, due mainly with module D. For the ODP, an impact, although minimal, is
to the water consumption and emissions into water that occur associated with module D since the steel recycling process has
during the manufacturing process. The higher impact of the a greater impact than the production process from raw
manufacturing process on these categories is mainly driven by materials.
the production of auxiliary materials (19 % of EP-freshwater
7. Requisite evidence
Not relevant for this EPD.
8. References
Standards Railway applications - Track - Rail - Part 4: Vignole railway rails
from 27 kg/m to, but excluding 46 kg/
AREMA 2022
Chapter 4 Rail. Manual for Railway Engineering EN 15804+A2
EN 15804:2012+A2:2019+AC:2021, Sustainability of
BS 11 : 1985 construction works — Environmental Product Declarations —
Specification for Railway Rails Core rules for the product category of construction products.
EN 13674-1:2011+A1:2017 ISO 14001
Railway applications – Track – Rail – Part 1: Vignole railway ISO 14001:2015. Environmental management systems -
rails 46 kg/m and above Requirements with guidance for use
EN 13674-2:2020 ISO 14025
Railway applications – Track – Rail – Part 2: Switch and EN ISO 14025:2011, Environmental labels and declarations —
crossing rails used in conjunction with Vignole railway rails 46 Type III environmental declarations — Principles and
kg/m and above procedures.
EN 13674-3:2006+A1:2010 ISO 45001
Railway applications – Track – Rail – Part 3: Check rails ISO 45001: 2018 Occupational health and safety management
systems -- Requirements with guidance for use
EN 13674-4 (edizione Aprile 2019)
6 Environmental Product Declaration - JSW Steel Italy Piombino S.p.A. - JSW steel rail
ISO 50001
ISO 50001: 2018, Energy management systems - EWC/AVV waste code
Requirements with guidance for use Directive governing introduction of the European Waste
Catalogue http://www.ngs-mbh.de/zs/eak.html
ISO 9001
ISO 9001:2015 Quality management systems- Requirements IBU 2021
Institut Bauen und Umwelt e.V.: General Instructions for the
UIC 860.O EPD programme of Institut Bauen und Umwelt e.V.,Version 2.0,
Techinical specification for the supply of rail. 9th edition, Berlin: Institut Bauen und Umwelt e.V., 2021, www.ibu-epd.com
January 2008
Managed LCA Content (formerly known as GaBi
Further References Databases)
Database for Life Cycle Engineering LBP, University of Stuttgart
Candidate list and Sphera, documentation of LCA for Expert (GaBi) 10 data
Candidate List of substances of very high concern for setshttps://sphera.com/life-cycle-assessment-lca-database/,
Authorisation published by the European Chemicals Agency in 2023
accordance with Article 59(10) of the REACH Regulation.
PCR Part A
CPR Product Category Rules for Building-Related Products and
Construction Production Regulation (EU) No 305/2011 of the Services, Part A: Calculation Rules for the Life Cycle
European Parliament and of the council of 9 March 2011 laying Assessment and Requirements on the Project report, Version
down harmonised conditions for the marketing of construction 1.1, Institut Bauen und Umwelt e.V., 01-2021
products and repealing Council Directive 89/106/EEC
PCR Part B
EPD Average of Finished Long Products (Steel) Product Category Rules for Construction Products, Part B:
Average of Finished Long Products (Steel) by JSW Steel Rails forming a track for vehicles, 08-2021
Limited. EPD registration number: S-P-04326. Publication date:
2021-10-21 https://environdec.com/library REACH Regulation
Regulation (EU) No 1907/2006 of the European Parliament and
EU Biocidal Products Regulation (No. 528/2012) of the Council of 18 December 2006 concerning the
The EU Biocidal Products Regulation (No. 528/2012) Guidance Registration, Evaluation, Authorisation and Restriction of
document for ASD industries (January 2016) Chemicals (REACH)
7 Environmental Product Declaration - JSW Steel Italy Piombino S.p.A. - JSW steel rail
Publisher
Institut Bauen und Umwelt e.V. +49 (0)30 3087748- 0
Hegelplatz 1 info@ibu-epd.com
10117 Berlin www.ibu-epd.com
Germany
Programme holder
Institut Bauen und Umwelt e.V. +49 (0)30 3087748- 0
Hegelplatz 1 info@ibu-epd.com
10117 Berlin www.ibu-epd.com
Germany
Author of the Life Cycle Assessment
Sphera Solutions GmbH +49 711 341817-0
Hauptstraße 111- 113 info@sphera.com
70771 Leinfelden-Echterdingen www.sphera.com
Germany
Owner of the Declaration
JSW Steel Italy Piombino +39 0565/64286
Largo Caduti sul Lavoro 21 a.merigo@jswitaly.com
57025 Piombino www.jswitaly.com
Italy
8 Environmental Product Declaration - JSW Steel Italy Piombino S.p.A. - JSW steel rail
