ENVIRONMENTAL PRODUCT DECLARATION
as per ISO 14025 and EN 15804+A2
Owner of the Declaration Kingspan Insulation B.V.
Programme holder Institut Bauen und Umwelt e.V. (IBU)
Publisher Institut Bauen und Umwelt e.V. (IBU)
Declaration number EPD-KSI-20210045-CBA1-EN
Issue date 12.03.2021
Valid to 11.03.2026
Kooltherm® K10
Kingspan Insulation B.V.
www.ibu-epd.com | https://epd-online.com
Umwelt Produktdeklaration Name des Herstellers – Name des Produkts
General Information
Kingspan Insulation B.V. Kooltherm® K10
Programme holder Owner of the declaration
IBU – Institut Bauen und Umwelt e.V. Kingspan Insulation B.V.
Panoramastr. 1 Lingewei 8
10178 Berlin 4004 LL Tiel
Germany The Netherlands
Declaration number Declared product / declared unit
EPD-KSI-20210045-CBA1-EN Kooltherm® K10 Soffit Board
1 m², 80 mm thickness, R = 4,0 m²·K/W
D
This declaration is based on the product Scope:
category rules: The insulation material Kooltherm® is produced by
Insulating materials made of foam plastics, 06.2017 Kingspan Insulation B.V. at the manufacturing facility in
(PCR checked and approved by the SVR) Tiel, the Netherlands. A glass tissue based facing is
autohesively bonded to the insulation core during
manufacture.
Issue date
12.03.2021
In order to enable the user of the EPD to calculate the
LCA results for different thicknesses, the EPD contains
Valid to
the respective calculation rules.
11.03.2026
The owner of the declaration shall be liable for the
underlying information and evidence; the IBU shall not
be liable with respect to manufacturer information, life
cycle assessment data and evidences.
The EPD was created according to the specifications
of EN 15804+A2. In the following, the standard will be
simplified as EN 15804.
Verification
The standard EN 15804 serves as the core PCR
Independent verification of the declaration and data
according to ISO 14025:2010
Dipl. Ing. Hans Peters internally x externally
(chairman of Institut Bauen und Umwelt e.V.)
Dr. Alexander Röder Dipl. Natw. ETH Sascha Iqbal
(Managing Director Institut Bauen und Umwelt e.V.)) (Independent verifier)
Product
Product description/Product definition
Kooltherm® K10 is a rigid thermoset cellular insulation Technical Data
material faced on both sides with a glass tissue based
facing. The product is available in variable thicknesses
from 20 mm up to 200 mm. This EPD is based on a Constructional data
thickness of 80 mm and R -value of 4,0 m²·K/W. Name Value Unit
D
For the placing on the market of the product in the Compressive strength acc. to EN
≥ 100 kPa
European Union/European Free Trade Association 13166
(EU/EFTA) (with the exception of Switzerland) Tensile strength perpendicular to
≥ 60 kPa
Regulation (EU) No. 305/2011 (CPR) applies. The faces acc. to EN 13166
product needs a declaration of performance taking into Thermal conductivity λd acc. to
0.021 W/(mK)
consideration EN 13166:2012+A2:2016 - Thermal EN 13166 for d = 20 – 44 mm
insulation products for buildings - Factory made Thermal conductivity λd acc. to
0.020 W/(mK)
phenolic foam (PF) products - specification and the EN 13166 for d = 45 – 120 mm
CE-marking. For the application and use the respective Thermal conductivity λd acc. to
0.021 W/(mK)
national provisions apply. EN 13166 for d = 121 – 159 mm
Thermal conductivity λd acc. to
Application EN 13166 for d = 160 – 200 mm 0.021 W/(mK)
Due to its high insulating value, Kooltherm® K10 is (2 layers)
suitable for use as soffit insulation.
2 Environmental Product Declaration Kingspan Insulation B.V. – Kooltherm® K10
Technical parameters not included are modulus of not classified as “hazardous products” according to
elasticity as well as sound absorption (not relevant for any current legislation, and can hence be declared as
this application) and creep (not placed under follows:
permanent load). - This article contains substances listed in the
candidate list (date: 19.01.2021) exceeding 0.1
Performance data of the product in accordance with percentage by mass: no.
the declaration of performance with respect to its - This article contains other carcinogenic, mutagenic,
essential characteristics according to EN reprotoxic (CMR) substances in categories 1A or 1B
13166:2012+A2:2016 - Thermal insulation products for which are not on the candidate list, exceeding 0.1
buildings - Factory made phenolic foam (PF) products - percentage by mass: no.
Specification - Biocide products were added to this construction
product or it has been treated with biocide products
Base materials/Ancillary materials (this then concerns a treated product as defined by the
The main materials are phenolic (PF) resin (between (EU) Biocidal Products Regulation No. 528/2012
70-80%) with added catalyst and additives (between (BPR): no.
15-20%). Phenolic rigid foam onto a facing material
(between 5-10%) is formed by the chemical reaction of The chemical functional group of the additives used in
these materials and adding a blowing agent with no the resin is that of non-ionic surfactants.
ozone depletion potential (ca. 5%). Due to the closed-
cell structure (conform EN 13166), the blowing agent Reference service life
remains in the foam. In the current REACH The reference service life is not to be declared in this
regulations, phenolic foam insulation products are EPD as it does not cover the use stage.
considered “articles” and are exempt from the
requirements of Article 57 and 59(1) of REACH
Regulation (EC) No 1907/2006. These products are
LCA: Calculation rules
Declared Unit waste state or disposal of final residues during the
The declared unit (1 m²) and conversion factors are construction process stage.
listed in the table below.
The end-of-life stage is a mandatory information
Declared unit module and it covers:
Name Value Unit · C1 de-construction, demolition;
Declared unit 1 m2 · C2 transport to waste processing;
Gross density 35 kg/m3 · C3 waste processing for reuse, recovery and/or
Conversion factor to 1 kg 2.8 kg/m2 recycling;
Grammage 2.8 kg/m2 · C4 disposal (not applicable for this EPD) including
Layer thickness 0.08 m provision and all transport, provision of all materials,
products and related energy and water use.
Environmental burden of the incineration (R1 > 60%)
System boundary of the product
Type of EPD: according to EN 15804: at the end-of-life stage are assigned to the product
cradle to gate with options, modules C1–C4, and system (C3); resulting potential credits for thermal and
module D (A1–A3, C, D and additional modules: electrical energy from energy substitution are declared
A4,A5). in module D.
According to PCR Part A: Renewable electricity sources for manufacturing
1a) declaration of one specific product from one plant All electricity used during production comes from
of one manufacturer; renewable sources.
By generating energy on-site with solar panels and
The product stage is a mandatory information module with procured energy from fully certified renewable
and it covers: sources. Following the global Net Zero Energy strategy
· A1, raw material extraction and processing, from Kingspan Group plc.
processing of secondary material input (e.g. recycling
processes), Comparability
· A2, transport to the manufacturer, Basically, a comparison or an evaluation of EPD data
· A3, manufacturing, including provision of all is only possible if all the data sets to be compared
materials, products and energy, packaging processing were created according to EN 15804 and the building
and its transport, as well as waste processing up to the context, respectively the product-specific
end-of-waste state or disposal of final residues during characteristics of performance, are taken into account.
the product stage.
Factors for different thicknesses
The construction process stage includes: The LCA results for the insulation material declared in
· A4 transport to the building site; this EPD refer to a product with a thickness of 80 mm.
· A5 installation in the building To enable the user of the EPD to calculate the results
including provision of all materials, products and for different thicknesses the factors in the following
energy, as well as waste processing up to the end-of- table can be used for the calculation. For modules A1-
3 Environmental Product Declaration Kingspan Insulation B.V. – Kooltherm® K10
A3, C3 and D the LCA results in chapter 5 have to be multiplied with these factors
Background data from GaBi software-system version 9
with Service Packs 39 GaBi ts is used.
LCA: Scenarios and additional technical information
Characteristic product properties
Information on biogenic Carbon Reuse, recovery and/or recycling potentials (D),
The total mass of biogenic carbon containing materials relevant scenario information
is less than 5 % of the total mass of the product and Waste incineration with energy recuperation is
accompanying packaging. assumed as end-of-life scenario
Technical information
The following technical information is a basis for the
declared modules or can be used for developing
specific scenarios in the context of a building
assessment.
Transport to the building site (A4)
Name Value Unit
Litres of fuel 0.0103 l/100km
Transport distance 100 km
Gross density of products transported 35 kg/m3
Installation into the building (A5)
Name Value Unit
Output substances following waste
0.06 kg
treatment on site packaging material
Within A1-A3 the following packaging of the final
product is included:
Polyethylene cover and wrap: 0,05 kg/m²
Others (mainly Expanded Polystyrene skid): 0,01
kg/m²
The recycling of the packaging is considered in A5.
End of life (C1-C4)
The assumptions for C1 are: diesel driven excavator
(100 kW; 0.2 litre fuel per ton excavated material).
The assumptions for C2 are: Truck Euro 6, diesel
driven, 26-28 t gross weight, assumed distance 50 km
Name Value Unit
Collected as mixed construction waste 2.8 kg
Energy recovery 2.8 kg
R1-value of waste incineration plant >60 %
4 Environmental Product Declaration Kingspan Insulation B.V. – Kooltherm® K10
LCA: Results
Disclaimer:
EP-freshwater: This indicator has been calculated as “kg P eq” as required in the characterization model
(EUTREND model, Struijs et al., 2009b, as implemented in ReCiPe;
http://eplca.jrc.ec.europa.eu/LCDN/developerEF.xhtml)
DESCRIPTION OF THE SYSTEM BOUNDARY (X = INCLUDED IN LCA; ND = MODULE OR INDICATOR NOT
DECLARED; MNR = MODULE NOT RELEVANT)
BENEFITS AND
CONSTRUCTI LOADS
PRODUCT STAGE ON PROCESS USE STAGE END OF LIFE STAGE BEYOND THE
STAGE SYSTEM
BOUNDARIES
5 Environmental Product Declaration Kingspan Insulation B.V. – Kooltherm® K10
lairetam
waR
ylppus tropsnarT
gnirutcafunaM
eht
morf
tropsnarT
etis
eht
ot
etag
ylbmessA esU
ecnanetniaM
riapeR
tnemecalpeR tnemhsibrufeR
ygrene
lanoitarepO esu
retaw
lanoitarepO esu
noitcurtsnoc-eD
noitilomed tropsnarT
gnissecorp
etsaW
lasopsiD -esueR -yrevoceR -gnilcyceR laitnetop
A1 A2 A3 A4 A5 B1 B2 B3 B4 B5 B6 B7 C1 C2 C3 C4 D
X X X X X ND ND MNR MNR MNR ND ND X X X X X
RESULTS OF THE LCA - ENVIRONMENTAL IMPACT according to EN 15804+A2: 1 m2 80 mm thickness
Core Indicator Unit A1-A3 A4 A5 C1 C2 C3 C4 D
GWP-total [kg CO2-Eq.] 5.63E+0 2.37E-2 1.60E-1 1.79E-3 1.19E-2 6.18E+0 0.00E+0 -2.66E+0
GWP-fossil [kg CO2-Eq.] 5.59E+0 2.35E-2 1.60E-1 1.79E-3 1.18E-2 6.18E+0 0.00E+0 -2.66E+0
GWP-biogenic [kg CO2-Eq.] -3.00E-2 -1.43E-4 -2.91E-6 -1.26E-7 -7.15E-5 2.77E-4 0.00E+0 -5.16E-3
GWP-luluc [kg CO2-Eq.] 6.45E-2 3.60E-4 5.76E-6 6.08E-8 1.80E-4 5.98E-5 0.00E+0 -1.81E-3
ODP [kg CFC11-Eq.] 1.11E-8 2.86E-18 4.77E-17 1.72E-19 1.43E-18 7.41E-16 0.00E+0 -2.72E-14
AP [mol H+-Eq.] 1.25E-2 2.78E-5 2.20E-5 8.52E-6 1.39E-5 3.69E-3 0.00E+0 -5.02E-3
EP-freshwater [kg PO4-Eq.] 1.79E-5 1.14E-7 8.42E-9 3.18E-10 5.68E-8 1.26E-7 0.00E+0 -3.50E-6
EP-marine [kg N-Eq.] 3.24E-3 8.57E-6 5.82E-6 3.98E-6 4.28E-6 1.77E-3 0.00E+0 -1.15E-3
EP-terrestrial [mol N-Eq.] 3.24E-2 1.00E-4 9.58E-5 4.36E-5 5.02E-5 2.04E-2 0.00E+0 -1.24E-2
POCP [kg NMVOC-Eq.] 1.42E-2 2.23E-5 1.67E-5 1.13E-5 1.12E-5 4.55E-3 0.00E+0 -3.31E-3
ADPE [kg Sb-Eq.] 5.35E-6 1.64E-9 6.88E-10 4.71E-11 8.19E-10 1.27E-8 0.00E+0 -4.15E-7
ADPF [MJ] 1.59E+2 3.14E-1 6.33E-2 2.43E-2 1.57E-1 1.67E+0 0.00E+0 -4.60E+1
[m³ world-Eq
WDP 9.48E-1 5.08E-4 1.66E-2 3.13E-6 2.54E-4 6.07E-1 0.00E+0 -2.47E-1
deprived]
GWP = Global warming potential; ODP = Depletion potential of the stratospheric ozone layer; AP = Acidification potential of land and water; EP =
Caption Eutrophication potential; POCP = Formation potential of tropospheric ozone photochemical oxidants; ADPE = Abiotic depletion potential for non-
fossil resources; ADPF = Abiotic depletion potential for fossil resources; WDP = Water (user) deprivation potential
RESULTS OF THE LCA - INDICATORS TO DESCRIBE RESOURCE USE according to EN 15804+A2: 1 m2
80 mm thickness
Indicator Unit A1-A3 A4 A5 C1 C2 C3 C4 D
PERE [MJ] 2.21E+1 1.82E-2 1.22E-2 7.14E-5 9.10E-3 2.22E-1 0.00E+0 -9.33E+0
PERM [MJ] 0.00E+0 0.00E+0 0.00E+0 0.00E+0 0.00E+0 0.00E+0 0.00E+0 0.00E+0
PERT [MJ] 2.21E+1 1.82E-2 1.22E-2 7.14E-5 9.10E-3 2.22E-1 0.00E+0 -9.33E+0
PENRE [MJ] 8.18E+1 3.14E-1 6.33E-2 2.43E-2 1.57E-1 7.84E+1 0.00E+0 -4.60E+1
PENRM [MJ] 7.67E+1 0.00E+0 0.00E+0 0.00E+0 0.00E+0 -7.67E+1 0.00E+0 0.00E+0
PENRT [MJ] 1.59E+2 3.14E-1 6.33E-2 2.43E-2 1.57E-1 1.67E+0 0.00E+0 -4.60E+1
SM [kg] 0.00E+0 0.00E+0 0.00E+0 0.00E+0 0.00E+0 0.00E+0 0.00E+0 0.00E+0
RSF [MJ] 0.00E+0 0.00E+0 0.00E+0 0.00E+0 0.00E+0 0.00E+0 0.00E+0 0.00E+0
NRSF [MJ] 0.00E+0 0.00E+0 0.00E+0 0.00E+0 0.00E+0 0.00E+0 0.00E+0 0.00E+0
FW [m³] 3.65E-2 3.08E-5 3.95E-4 1.66E-7 1.93E-5 1.79E-2 0.00E+0 -1.10E-2
PERE = Use of renewable primary energy excluding renewable primary energy resources used as raw materials; PERM = Use of
renewable primary energy resources used as raw materials; PERT = Total use of renewable primary energy resources; PENRE = Use of
non-renewable primary energy excluding non-renewable primary energy resources used as raw materials; PENRM = Use of non-
Caption
renewable primary energy resources used as raw materials; PENRT = Total use of non-renewable primary energy resources; SM = Use
of secondary material; RSF = Use of renewable secondary fuels; NRSF = Use of non-renewable secondary fuels; FW = Use of net fresh
water
RESULTS OF THE LCA – WASTE CATEGORIES AND OUTPUT FLOWS according to EN 15804+A2:
1 m2 80 mm thickness
Indicator Unit A1-A3 A4 A5 C1 C2 C3 C4 D
HWD [kg] 7.52E-5 1.75E-8 2.96E-10 2.57E-12 8.76E-9 1.06E-9 0.00E+0 -1.89E-8
NHWD [kg] 7.48E-2 2.55E-5 1.54E-2 1.45E-7 1.28E-5 3.11E-2 0.00E+0 -1.99E-2
RWD [kg] 1.74E-3 4.26E-7 2.91E-6 2.79E-8 2.13E-7 7.51E-5 0.00E+0 -3.72E-3
CRU [kg] 0.00E+0 0.00E+0 0.00E+0 0.00E+0 0.00E+0 0.00E+0 0.00E+0 0.00E+0
MFR [kg] 0.00E+0 0.00E+0 0.00E+0 0.00E+0 0.00E+0 0.00E+0 0.00E+0 0.00E+0
MER [kg] 0.00E+0 0.00E+0 6.39E-2 0.00E+0 0.00E+0 2.80E+0 0.00E+0 0.00E+0
EEE [MJ] 0.00E+0 0.00E+0 3.54E-1 0.00E+0 0.00E+0 1.07E+1 0.00E+0 0.00E+0
EET [MJ] 0.00E+0 0.00E+0 6.38E-1 0.00E+0 0.00E+0 1.91E+1 0.00E+0 0.00E+0
HWD = Hazardous waste disposed; NHWD = Non-hazardous waste disposed; RWD = Radioactive waste disposed; CRU = Components
Caption for re-use; MFR = Materials for recycling; MER = Materials for energy recovery; EEE = Exported electrical energy; EEE = Exported
thermal energy
RESULTS OF THE LCA – additional impact categories according to EN 15804+A2-optional:
1 m2 80 mm thickness
Indicator Unit A1-A3 A4 A5 C1 C2 C3 C4 D
[Disease
PM 1.21E-7 1.60E-10 3.02E-10 9.53E-11 7.99E-11 1.05E-8 0.00E+0 -4.26E-8
Incidence]
[kBq U235-
IR 2.72E-1 6.24E-5 3.86E-4 4.08E-6 3.12E-5 1.17E-2 0.00E+0 -6.10E-1
Eq.]
ETP-fw [CTUe] 5.48E+1 2.11E-1 4.48E-2 1.64E-2 1.06E-1 5.65E-1 0.00E+0 -1.02E+1
HTP-c [CTUh] 6.33E-9 4.24E-12 3.42E-12 2.79E-13 2.12E-12 9.57E-11 0.00E+0 -1.88E-9
HTP-nc [CTUh] 6.14E-8 1.70E-10 2.51E-10 9.74E-12 8.52E-11 1.11E-9 0.00E+0 -9.42E-9
SQP [-] 9.55E+0 1.41E-1 1.59E-2 6.36E-5 7.07E-2 3.28E-1 0.00E+0 -6.93E+0
PM = Potential incidence of disease due to PM emissions; IR = Potential Human exposure efficiency relative to U235; ETP-fw = Potential
Caption comparative Toxic Unit for ecosystems; HTP-c = Potential comparative Toxic Unit for humans (cancerogenic); HTP-nc = Potential
comparative Toxic Unit for humans (not cancerogenic); SQP = Potential soil quality index
Disclaimer 1 – for the indicator IR
This impact category deals mainly with the eventual impact of low dose ionizing radiation on human health of the
nuclear fuel cycle. It does not consider effects due to possible nuclear accidents, occupational exposure nor due
to radioactive waste disposal in underground facilities. Potential ionizing radiation from the soil, from radon and
from some construction materials is also not measured by this indicator.
Disclaimer 2 – for the indicators ADPE, ADPF, WDP, ETP-fw, HTP-c, HTP-nc, SQP
The results of this environmental impact indicator shall be used with care as the uncertainties on these results are
high or as there is limited experienced with the indicator.
References
EN 13166
EN 13166:2012+A2:2016: Thermal insulation products LCA-tool
for buildings. Factory made phenolic foam (PF) Kingspan LCA tool, version 1.0. IBU-KSI-202001-LT1-
products. Specification EN.
Developed by Sphera Solutions GmbH (formely
EN 15804+A2 Thinkstep GmbH)
EN15804/A2: Sustainability of construction works -
Environmental product declarations - Core rules for the PCR Version 1.7, Part A
product category of construction products, 2019 Institut Bauen und Umwelt e.V., Berlin (pub.): Product
Category Rules for Building-Related Products and
BPR services, Part A: Calculation Rules for the Life Cycle
Regulation (EU) No 528/2012 of the European Assessment and Requirements on the Project Report ,
Parliament and of the Council of 22 May 2012 March 2018
concerning the making available on the market and
use of biocidal products PCR 2017, Part B
Institut Bauen und Umwelt e.V., Berlin (pub.): Product
CPR Category Rules for Construction Products from the
Regulation (EU) No. 305/2011 of the European range of Environmental Product Declarations of Institut
Parliament and of the Council of 9 March 2011 laying Bauen und Umwelt (IBU), Part B: Requirements on the
down harmonised condition for the marketing of EPD for insulating materials made of foam
construction products and repealing Council Directive plastics.June 2017
89/106/EC
REACH
GaBi ts Regulation (EC) No 1907/2006 of the European
thinkstep AG: Leinfelden-Echterdingen GaBi Software- Parliament and of the Council on the Registration,
System and Database for Life Cycle Engineering 1992- Evaluation, Authorisation and Restriction of Chemicals
2019 (REACH)
https://echa.europa.eu/candidate-list-table; accessed
IBU 2016 19th of January 2021, 211 substances listed.
IBU (2016): General Programme Instructions for the
Preparation of EPDs at the Institut Bauen und Umwelt Renewable Energy Certificate
e.V., Version 1.1 Institut Bauen und Umwelt e.V., Towarowa Gielda Energii S.A.: Guarantees of origin
Berlin, www.ibu-epd.de Document ID: RGP_ACTBV_2019-12-31_0720
ISO 14025
EN ISO 14025:2011-10 - Environmental labels and
declarations — Type III environmental declarations —
Principles and procedures
6 Environmental Product Declaration Kingspan Insulation B.V. – Kooltherm® K10
Publisher
Institut Bauen und Umwelt e.V. Tel +49 (0)30 3087748- 0
Panoramastr. 1 Fax +49 (0)30 3087748- 29
10178 Berlin Mail info@ibu-epd.com
Germany Web www.ibu-epd.com
Programme holder
Institut Bauen und Umwelt e.V. Tel +49 (0)30 - 3087748- 0
Panoramastr 1 Fax +49 (0)30 – 3087748 - 29
10178 Berlin Mail info@ibu-epd.com
Germany Web www.ibu-epd.com
Author of the Life Cycle
Assessment Tel +31 (0) 543 543 210
Kingspan Insulation B.V. Fax +31 (0) 344 675 251
Lingewei 8 Mail info@kingspaninsulation.nl
4004LL Tiel Web www.kingspan.com
Netherlands
Owner of the Declaration
Kingspan Insulation B.V. Tel +31 (0) 543 543 210
Lingewei 8 Fax +31 (0) 344 675 251
4004LL Tiel Mail info@kingspaninsulation.nl
Netherlands Web www.kingspan.com
