ENVIRONMENTAL PRODUCT DECLARATION
as per ISO 14025 and EN 15804+A2
Owner of the Declaration Leviat GmbH
Publisher Institut Bauen und Umwelt e.V. (IBU)
Programme holder Institut Bauen und Umwelt e.V. (IBU)
Declaration number EPD-HAL-20230141-IBC1-EN
Issue date 11.08.2023
Valid to 10.08.2028
HALFEN mounting and cast-in anchor channel systems
Leviat GmbH
www.ibu-epd.com | https://epd-online.com
1. General Information
Leviat GmbH HALFEN mounting and cast-in anchor channel
systems
Programme holder Owner of the declaration
IBU – Institut Bauen und Umwelt e.V. Leviat GmbH
Hegelplatz 1 Liebigstrasse 14
10117 Berlin 40764 Langenfeld
Germany Germany
Declaration number Declared product / declared unit
EPD-HAL-20230141-IBC1-EN The declared unit is one running metre of anchor channel with a weight of
2.69 kg per meter.
This declaration is based on the product category rules: Scope:
Thin walled profiles and profiled panels of metal, 01.08.2021 The results declared in this document and its annexe are based on the
(PCR checked and approved by the SVR) product HTA-CE (HTA) 40/22 with HS 40/22 channel bolts with a weight of
2,69 kg/m. The data in the annexe can be used to calculate all other
variants of HALFEN cast-in anchor channel systems HTA-CE (HTA), HZA,
Issue date and HZA-PS as well as HALFEN mounting channels HM, HZM with
corresponding HS and HZS channel bolts (hook-head channel bolts and
11.08.2023
hammer-head channel bolts). HALFEN channels are produced from
carbon or stainless steel. HALFEN cast-in anchor channels type HTA-CE,
HZA, and HZA-PS as well as HALFEN mounting channels HM, HZM are
Valid to
produced at Leviat manufacturing plant Langenfeld/Germany and HALFEN
10.08.2028 cast-in anchor channels type HTA and HZA are produced at Leviat
manufacturing plant Converse/USA. More than 97 % of the production
happens in Germany.
Specific data from the Leviat production facility in Langenfeld/Germany
was recorded for the LCA. The results of this EPD can be used as
approximation for the products mentioned above produced in the
production facility of Converse/USA.
The owner of the declaration shall be liable for the underlying information
and evidence; the IBU shall not be liable with respect to manufacturer
information, life cycle assessment data and evidences.
The EPD was created according to the specifications of EN 15804+A2. In
the following, the standard will be simplified as EN 15804.
Dipl.-Ing. Hans Peters
(Chairman of Institut Bauen und Umwelt e.V.)
Verification
The standard EN 15804 serves as the core PCR
Independent verification of the declaration and data according to ISO
14025:2011
internally X externally
Florian Pronold Matthias Klingler,
(Managing Director Institut Bauen und Umwelt e.V.) (Independent verifier)
1 Environmental Product Declaration - Leviat GmbH - HALFEN mounting and cast-in anchor channel systems
2. Product
2.1 Product description/Product definition 2.2 Application
The product portfolio of HALFEN channels compromises cast-in HALFEN mounting and anchor channels ensure the transfer of
anchor channels type HTA-CE/HTA, HZA, and HZA-PS as well high loads to steel structures or in reinforced and unreinforced
as HALFEN mounting channels HM and HZM (welded or fixed concrete components.
to a substructure) with corresponding hook-head channel bolts
and hammerhead channel bolts named as HS (for HTA- Mounting channels can be screwed or welded directly to the
CE/HTA and HM) and HZS (for HZA and HZM). component or substructure.
HALFEN mounting and anchor channels comprise a C-shaped Cast-in anchor channels are cast in concrete. Prior to the
steel profile made of carbon or stainless steel with casting process, they are positioned in the component and
corresponding channel bolts; HALFEN mounting channels are fastened in their position to the formwork, to the reinforcement
also available in mill finish. or by appropriate auxiliary construction. HALFEN channels
HALFEN cast-in anchor channels additionally consist of at least serve towards subsequent fastening of fixtures.
two mounted anchors on the channel back.
Typical areas of application include curtain wall façades,
These anchors are formed as round bolt anchors or as I- fastening elevator installations in shafts, fastening of overhead
anchors. The anchors are mounted on the channel back by wires, utility service pipes and cables in tunnels, fastening of
riveting or welding process. Hot-dipped galvanized quality and handrails, platforms or seats, connection of precast concrete
stainless steel were considered for this EPD. elements, supporting structures for pipes as well as
applications in the area of installation technology.
The inner section of the anchor channel is filled with PE foam
which prevents an entry of concrete slurry during casting. 2.3 Technical Data
All geometrical dimensions, product-specific parameters and
The various HALFEN channels differ in terms of mass in the static load capacities of the different mounting and cast-in
relation to running meters (1.08 kg/m- 12.19 kg/m). The anchor channel systems HTA-CE/HTA/HM, HZA/HZM and
declared reference product is the cast-in anchor channel HZA-PS are given in the following technical specifications:
system HTA-CE (HTA) 40/22 with HS 40/22 channel bolts with
a weight of 2.69 kg/m.
HTA-CE/HTA/HM system:
The LCA results can be applied to the following HALFEN
channel types (mounting and cast-in anchor channels) by ETA 09/0339
approximately scaling the mass to the specific product weight
by using the data in the EPD and the annexe: ETA 19/0438
ICC-ESR 1008 by ICC-ES
• HTA-CE / HTA / HM 28/15
• HTA-CE / HTA / HM 38/17
• HTA-CE / HTA / HM 40/25
HZA and HZA-PS system:
• HTA-CE / HTA / HM 40/22
• HTA-CE / HTA 40/22P
ETA-20/1081
• HTA-CE / HTA / HM 49/30
• HTA-CE / HTA / HM 50/30
ETA-17/0728
• HTA-CE / HTA 50/30P
• HTA-CE / HTA / HM 54/33
ICC-ESR 4016 by ICC-ES
• HTA-CE / HTA / HM 52/34
• HTA-CE / HTA / HM 55/42
• HTA-CE / HTA / HM 72/48
Some types of cast-in anchor channels HTA-CE/HTA, HZA and
• HZA / HZM 41/22
HZA-PS are also approved for fatigue cyclic tension loads,
• HZA / HZM 29/20
seismic loading and exposure to fire. Please refer to the
• HZA / HZM 38/23
mentioned approval documents for a detailed design of the
• HZA / HZM 41/27
anchor channel and other data related to the specific
• HZA / HZM 53/34
application condition.
• HZA / HZM 64/44
• HZA-PS 29/20 Technical constructional data HTA-CE (HTA) 40/22
• HZA-PS 38/23 Name Value Unit
• HZA-PS 41/27
Minimum anchoring depth min h(ef) 79 mm
• HZA-PS 53/34
Minimum edge distance c(min) 50 mm
• HZA-PS 64/44
Anchor channel width b(ch) 39.5 mm
For the placing of the product on the market in the European Anchor channel height h(ch) 23 mm
Union/European Free Trade Association (EU/EFTA) (with the Profile thickness t[nom] 2.6 mm
exception of Switzerland) the Regulation (EU) No. 305/2011
Performance data of the product in accordance with the
(CPR) applies. Products with an ETA need a declaration of
declaration of performance with respect to its essential
performance and the CE-marking. For the application and use
characteristics according to the respective ETA.
the respective national provisions apply.
2 Environmental Product Declaration - Leviat GmbH - HALFEN mounting and cast-in anchor channel systems
2.4 Delivery status 2.8 Product processing/Installation
HALFEN mounting and cast-in anchor channels and HALFEN The HALFEN mounting channel systems HM/HZM and cast-in
channel bolts are packed separately and can also be ordered anchor channel systems HTA-CE/HTA/HZA/HZA-PS are
separately (further information available in section 2.9). supplied as a ready-to-install channel element. The HALFEN
cast-in anchor channel is positioned in the building shell or in
2.5 Base materials/Ancillary materials the precast concrete
Name Value Unit plant during or alternatively after the reinforcement installation
Channel profile: galvanized steel 82 % without the use of lifting equipment. The HALFEN cast-in
anchor channel is positioned in the component and fastened in
Channel anchor: galvanized steel 6 %
position to the formwork, to the reinforcement or by appropriate
Channel bolt set: galvanized steel 11 %
auxiliary construction and secured against slippage during
Channel Filler: PE Foam 1 % subsequent concreting. After installation and casting, the foam
The product weight with respect to the declared unit HTA-CE is usually removed and disposed of.
(HTA) 40/22 in hot-dipped galvanized quality is ca. 2.69 kg per HALFEN mounting channels are directly welded or screwed to
metre (average value). the substructure.
This product/at least one partial article contains substances No special environmental protection measures need to be
listed in the candidate list (17.01.2023) exceeding 0.1 taken while processing HALFEN mounting or cast-in channels.
percentage by mass: no.
2.9 Packaging
This product/at least one partial article contains other
The HALFEN mounting and cast-in channels are delivered
carcinogenic, mutagenic, reprotoxic (CMR) substances in
packed and strapped in bundles as long goods.
categories 1A or 1B which are not on the candidate list,
Up to a length of 1.05 metres, mounting and cast-in channels
exceeding 0.1 percentage by mass: no.
are delivered on Euro pallets or cardboard. Depending on the
Biocide products were added to this construction product or it
size and length, HALFEN channel bolts are packed in packing
has been treated with biocide products (this then concerns a
units of several sizes in cardboard boxes.
treated product as defined by the (EU) Ordinance on Biocide
The individual packaging materials should be separated
Products No. 528/2012): no
according to their type and recycled.
2.6 Manufacture
2.10 Condition of use
The materials needed for the final assembly of the HALFEN
All supplied materials are protected in the installed condition
mounting and cast-in anchor channel systems HTA-
against external influences and designed for the service life of
CE/HTA/HM and HZA/HZA-PS/HZM are manufactured in-
the respective construction.
house or purchased from qualified vendors.
The HALFEN mounting and cast-in anchor channels are made
2.11 Environment and health during use
of cold-formed or hot-rolled channel profiles. The cold-formed
When used as designated, there is no impact on the
channel profiles are produced at LEVIAT plant
environment or health. No risks can arise to water, air and soil if
Langenfeld/Germany. The anchors are mounted on the channel
the products are used as designated.
back by a riveting or welding process. HALFEN cast-in anchor
channels with riveted bolt anchors are produced at LEVIAT 2.12 Reference service life
plant Langenfeld/Germany. HALFEN cast-in anchor channels
A service life of at least 50 years confirmed by approval
with welded I-anchors are produced at LEVIAT plant
procedures is applicable for HALFEN mounting and cast-in
Langenfeld/Germany and LEVIAT plant Converse/USA.
channel systems HM/HZM and HTA-CE/HTA/HZA/HZA-PS,
The anchor channels made of carbon steel are hot-dipped
which are in line with the safety concepts outlined in the
galvanised after the mounting process of the anchors. The filler
Eurocode or ACI. The practical service life can however be
is assembled after the galvanising process at LEVIAT plant
considerably longer. A further condition for the service life is
Langenfeld/Germany or LEVIAT plant Converse/USA.
that the HALFEN mounting and cast-in channel system is used
in accordance with the designed application. This service life
2.7 Environment and health during manufacturing
refers to a static design approach and not to reference service
The criteria for environmental and energy management and the
life according to ISO 15686.
requirements for Health and Safety at work follow all
Description of the influences on the ageing of the product when
statutory requirements and LEVIAT standards.
applied in accordance with the rules of technology.
LEVIAT is certified according to DIN EN ISO 50001 for all its 18
locations inside Europe, the United States of America and 2.13 Extraordinary effects
China by the SWEDAC Certification Institute International
Fire
GmbH.
HALFEN mounting channel systems HM/HZM and cast-in
Since 1994 all former HALFEN locations are certified according
channel systems HTA-CE/HTA/HZA/HZA-PS correspond to
to ISO 9001 (ISO 9001:2015).
building material class A1 according to EN 13501. In addition,
HALFEN cast-in channel systems are approved for fire
The continuous production and product quality according to the
exposure (see section 2.3).
product specifications and approval specifications of HALFEN
Fire protection
mounting and cast-in anchor channel systems are ensured by
an in-process quality control by LEVIAT and by regularly third- Name Value
party quality inspections by MPA NRW and IAS certified bodies. Building material class A1
All types of waste such as steel, PE foam, wood (wood pallets)
Burning droplets
and packaging materials (cardboard) that are incurred in the
Smoke gas development
production of the product or remain as excess material will be
separated according to type and recycled.
3 Environmental Product Declaration - Leviat GmbH - HALFEN mounting and cast-in anchor channel systems
recycled into the material cycle.
Water In view of an efficient recycling process it should be ensured
The declared HALFEN mounting and cast-in anchor channel that a separation of materials during decommissioning is
systems comprise hot-dipped galvanised and stainless steel. possible.
There are no environmental risks attributable to the effects of
water. 2.15 Disposal
The disposal of non-recycled parts of HALFEN mounting and
Mechanical destruction cast-in anchor channels can be disposed of at any waste
In the event of unintentional mechanical destruction, there is no disposal site with the appropriate waste number EWC 191001
risk for users or the environment if the product has been (for steel components) or EWC 170904 (other components)
installed correctly. according to the European Waste Code of the European Waste
Catalogue.
2.14 Re-use phase
HALFEN mounting and cast-in anchor channels cannot be re- 2.16 Further information
used but material recycling is possible. www.leviat.com
All components of the described product can be returned and
3. LCA: Calculation rules
3.1 Declared Unit 3.3 Estimates and assumptions
The declared unit is 1 m length of cast-in anchor channel. No estimates and assumptions were made.
Declared unit
3.4 Cut-off criteria
Name Value Unit In this assessment, all data for the production process is
Declared unit 1 m considered. This includes input flows with a contribution of less
Grammage 2.69 kg/m than 1 % of mass or energy. The transport expenditure for all
raw materials is considered. Impacts relating to the production
More than 97 % of the production happens in Germany.
of machines and facilities required during production are
Specific data from the Leviat production facility in
outside the scope of this assessment.
Langenfeld/Germany was recorded for the LCA.
The impacts arising from the dismantling of the products from
the building structure (separating concrete, metal and other
The results of this EPD can be used as an approximation for
building materials) are not considered. The impacts are
the products mentioned above produced in the production
estimated to contribute less than 1 % to the overall result.
facility of Converse/USA.
Production of capital equipment, facilities and infrastructure
3.2 System boundary required for manufacture are outside the scope of this
assessment.
Type of the EPD: cradle-to-gate - with options, modules C1-C4
and module D (A1-A3 + C + D and additional modules: A4, A5).
Transport processes for the packaging materials are neglected.
Production Stage (A1-A3): The Product stage includes:
The impacts are estimated to contribute less than 1 % to the
· A1 Raw material supply and processing (mainly steel),
overall result.
· A2 Transport of raw materials to the manufacturer,
· A3 Production of HTA-CE (HTA) 40/22 with HS 40/22 channel
3.5 Background data
bolts in the factory, (incl. energy provision for welding and
For modelling the life cycle of the declared product, the Life
riveting, treatment of production waste, production of packaging
Cycle Assessment software GaBi developed by Sphera GmbH
materials).
is used.
Construction stage (A4-A5): The construction process stage
The underlying database is GaBi 2022, version 2022.2
includes:
· A4 transport to the construction site 100km by truck,
· A5 Disposal of the packaging after installation of the HTA-CE 3.6 Data quality
(HTA) 40/22 with HS 40/22 channel bolts
The data quality can be described as good. The primary data
collection was done thoroughly, all flows were considered.
End-of-life stage (C1-C4): The end-of-life stage includes:
Technological, geographical and temporal representativeness is
· C1 machine-assisted de-construction (demolition excavator -
given. Primary data to the year 2021. The background data
diesel-powered)
have been taken from the GaBi databases. The last update of
· C2 transport to waste processing; 50 km by truck.
the databases has taken place in 2022.
Transport distance can be adjusted at building level if
necessary (e.g., for 100 km
actual transport distance: multiply LCA values by factor 2) 3.7 Period under review
· C3 waste processing for incineration of plastic components, The period under review is the year 2021.
recycling of metals
· C4 no components of the product are landfilled.
3.8 Geographic Representativeness
Benefits and loads beyond the System Boundary Land or region, in which the declared product system is
(D): Module D includes: manufactured, used or handled at the end of the product´s
Material recovery potentials from metal recycling and energy lifespan: Europe
recovery potentials from the
thermal recovery of the mixed plastic waste.
4 Environmental Product Declaration - Leviat GmbH - HALFEN mounting and cast-in anchor channel systems
3.9 Allocation 3.10 Comparability
Information about allocation procedure of single datasets is Basically, a comparison or an evaluation of EPD data is only
documented in https://gabi.sphera.com/databases/gabi-data- possible if all the data sets to be compared were created
search/ according to EN 15804 and the building context, respectively
Allocation in the foreground data: The production process does the product-specific characteristics of performance, are taken
not deliver any co-products. The applied software model does into account. The used database is GaBi 2022, version 2022.2.
not contain any allocation.
4. LCA: Scenarios and additional technical information
Credits for potential avoided burdens due to energy substitution
Characteristic product properties of biogenic carbon of electricity
and thermal energy generation are declared in module D and
affects only the
Information on describing the biogenic Carbon Content at rate of primary material (no secondary materials).
factory gate Name ValueUnit
Name ValueUnit Output substances following waste treatment on
0.04 kg
kg site (pallets and cartons)
Biogenic carbon content in product -
C
Biogenic carbon content in accompanying kg
0.016
packaging C
End of life (C1-C4)
The product dismantling from the building is done with a
machine.
Name Value Unit
Transport to the building site (A4) Recycling 2.67 kg
Name Value Unit Energy recovery 0.019 kg
Transport distance 100 km
Reuse, recovery and/or recycling potentials (D), relevant
scenario information
Assembly (A5)
Collection rate is 100 %
Module A5 includes the treatment and disposal of packaging
material.
5 Environmental Product Declaration - Leviat GmbH - HALFEN mounting and cast-in anchor channel systems
5. LCA: Results
DESCRIPTION OF THE SYSTEM BOUNDARY (X = INCLUDED IN LCA; ND = MODULE OR INDICATOR NOT DECLARED; MNR =
MODULE NOT RELEVANT)
Benefits and
Construction loads beyond
Product stage Use stage End of life stage
process stage the system
boundaries
la ire ta m w a Ry lp p u s tro p s n a rT g n iru tc a fu n a M e h t m o rf tro p s n a rTe tis e h t o t e ta g y lb m e s s A e s U e c n a n e tn ia M ria p e R tn e m e c a lp e R tn e m h s ib ru fe R y g re n e la n o ita re p Oe s u re ta w la n o ita re p Oe s u n o itc u rts n o c -e Dn o itilo m e d tro p s n a rT g n is s e c o rp e ts a W la s o p s iD -e s u e R-y re v o c e R-g n ilc y c e Rla itn e to p
A1 A2 A3 A4 A5 B1 B2 B3 B4 B5 B6 B7 C1 C2 C3 C4 D
X X X X X MND MND MNR MNR MNR MND MND X X X MND X
RESULTS OF THE LCA - ENVIRONMENTAL IMPACT according to EN 15804+A2: HTA-CE (HTA) 40/22 with HS 40/22 channel
bolts with a weight of 2.6 kg/m
Parameter Unit A1-A3 A1 A2 A3 A4 A5 C1 C2 C3 D
GWP-total kg CO 2 eq 3.62E+00 1.81E-02 6.26E-02 3.62E+00 1.81E-02 6.26E-02 1.76E-03 9.18E-03 5.92E-02 -1.04E+00
GWP-fossil kg CO 2 eq 3.66E+00 1.79E-02 1.04E-03 3.66E+00 1.79E-02 1.04E-03 1.75E-03 8.97E-03 5.92E-02 -1.04E+00
GWP-
biogenic kg CO 2 eq -5E-02 5.84E-05 6.15E-02 -5E-02 5.84E-05 6.15E-02 0 1.46E-04 1.9E-06 -1.71E-04
GWP-luluc kg CO 2 eq 8.06E-04 1.21E-04 1.37E-07 8.06E-04 1.21E-04 1.37E-07 1.13E-05 6.06E-05 6.24E-08 -1.52E-04
ODP kg CFC11 eq 1.38E-11 1.77E-15 5.43E-15 1.38E-11 1.77E-15 5.43E-15 1.65E-16 8.83E-16 2.54E-15 -1.28E-12
AP mol H+ eq 8.59E-03 2.02E-05 1.02E-05 8.59E-03 2.02E-05 1.02E-05 8.47E-06 1.01E-05 5.88E-06 -3.18E-03
EP-
kg P eq 5.02E-06 6.42E-08 1.3E-09 5.02E-06 6.42E-08 1.3E-09 6.01E-09 3.21E-08 5.91E-10 -9.23E-07
freshwater
EP-marine kg N eq 2E-03 6.51E-06 3.35E-06 2E-03 6.51E-06 3.35E-06 3.96E-06 3.26E-06 1.23E-06 -4.93E-04
EP-terrestrial mol N eq 2.15E-02 7.8E-05 4.87E-05 2.15E-02 7.8E-05 4.87E-05 4.39E-05 3.9E-05 2.75E-05 -4.81E-03
kg NMVOC
POCP 6.82E-03 1.74E-05 9.09E-06 6.82E-03 1.74E-05 9.09E-06 1.11E-05 8.69E-06 3.65E-06 -1.86E-03
eq
ADPE kg Sb eq 1.23E-04 1.81E-09 1.32E-10 1.23E-04 1.81E-09 1.32E-10 1.7E-10 9.06E-10 6.14E-11 -1.11E-04
ADPF MJ 4.57E+01 2.36E-01 1.5E-02 4.57E+01 2.36E-01 1.5E-02 2.21E-02 1.18E-01 6.9E-03 -1.11E+01
m3 world eq
WDP 2.51E-01 2.01E-04 7.5E-03 2.51E-01 2.01E-04 7.5E-03 1.88E-05 1.01E-04 5.46E-03 -2.11E-01
deprived
GWP = Global warming potential; ODP = Depletion potential of the stratospheric ozone layer; AP = Acidification potential of land and water; EP =
Eutrophication potential; POCP = Formation potential of tropospheric ozone photochemical oxidants; ADPE = Abiotic depletion potential for non-fossil
resources; ADPF = Abiotic depletion potential for fossil resources; WDP = Water (user) deprivation potential)
RESULTS OF THE LCA - INDICATORS TO DESCRIBE RESOURCE USE according to EN 15804+A2: HTA-CE (HTA) 40/22 with
HS 40/22 channel bolts with a weight of 2.6 kg/m
Parameter Unit A1-A3 A1 A2 A3 A4 A5 C1 C2 C3 D
PERE MJ 8.42E+00 1.64E-02 6.09E-01 8.42E+00 1.64E-02 6.09E-01 1.53E-03 8.18E-03 1.63E-03 -6E-01
PERM MJ 6.06E-01 0 -6.06E-01 6.06E-01 0 -6.06E-01 0 0 0 0
PERT MJ 9.03E+00 1.64E-02 3.47E-03 9.03E+00 1.64E-02 3E-03 1.53E-03 8.18E-03 1.63E-03 -6E-01
PENRE MJ 4.49E+01 2.37E-01 1.5E-02 4.49E+01 2.37E-01 1.5E-02 2.22E-02 1.19E-01 8.76E-01 -1.11E+01
PENRM MJ 8.69E-01 0 0 8.69E-01 0 0 0 0 -8.69E-01 0
PENRT MJ 4.58E+01 2.37E-01 1.5E-02 4.58E+01 2.37E-01 1.5E-02 2.22E-02 1.19E-01 6.9E-03 -1.11E+01
SM kg 2.21E+00 0 0 2.21E+00 0 0 0 0 0 4.77E-01
RSF MJ 0 0 0 0 0 0 0 0 0 0
NRSF MJ 0 0 0 0 0 0 0 0 0 0
FW m3 1.15E-02 1.89E-05 1.76E-04 1.15E-02 1.89E-05 1.76E-04 1.77E-06 9.45E-06 1.28E-04 -5.35E-03
PERE = Use of renewable primary energy excluding renewable primary energy resources used as raw materials; PERM = Use of renewable primary
energy resources used as raw materials; PERT = Total use of renewable primary energy resources; PENRE = Use of non-renewable primary energy
excluding non-renewable primary energy resources used as raw materials; PENRM = Use of non-renewable primary energy resources used as raw
materials; PENRT = Total use of non-renewable primary energy resources; SM = Use of secondary material; RSF = Use of renewable secondary fuels;
NRSF = Use of non-renewable secondary fuels; FW = Use of net fresh water
RESULTS OF THE LCA – WASTE CATEGORIES AND OUTPUT FLOWS according to EN 15804+A2:
HTA-CE (HTA) 40/22 with HS 40/22 channel bolts with a weight of 2.6 kg/m
Parameter Unit A1-A3 A1 A2 A3 A4 A5 C1 C2 C3 D
HWD kg 5.25E-09 1.25E-12 1.45E-12 5.25E-09 1.25E-12 1.45E-12 1.17E-13 6.27E-13 6.49E-13 -3.82E-10
NHWD kg 3.8E-02 3.86E-05 5.2E-04 3.8E-02 3.86E-05 5.2E-04 3.61E-06 1.93E-05 2.35E-04 9.64E-02
RWD kg 2.47E-03 4.4E-07 8.87E-07 2.47E-03 4.4E-07 8.87E-07 4.12E-08 2.2E-07 4.17E-07 -2.61E-04
CRU kg 0 0 0 0 0 0 0 0 0 0
6 Environmental Product Declaration - Leviat GmbH - HALFEN mounting and cast-in anchor channel systems
MFR kg 1.16E-02 0 0 1.16E-02 0 0 0 0 2.68E+00 0
MER kg 0 0 0 0 0 0 0 0 0 0
EEE MJ 2.53E-03 0 1.05E-01 2.53E-03 0 1.05E-01 0 0 1.26E-01 0
EET MJ 4.49E-03 0 1.88E-01 4.49E-03 0 1.88E-01 0 0 2.25E-01 0
HWD = Hazardous waste disposed; NHWD = Non-hazardous waste disposed; RWD = Radioactive waste disposed; CRU = Components for re-use;
MFR = Materials for recycling; MER = Materials for energy recovery; EEE = Exported electrical energy; EET = Exported thermal energy
RESULTS OF THE LCA – additional impact categories according to EN 15804+A2-optional:
HTA-CE (HTA) 40/22 with HS 40/22 channel bolts with a weight of 2.6 kg/m
Parameter Unit A1-A3 A1 A2 A3 A4 A5 C1 C2 C3 D
Disease
PM 1.16E-07 1.38E-10 5.03E-11 1.16E-07 1.38E-10 5.03E-11 9.61E-11 6.92E-11 3.43E-11 -4.37E-08
incidence
IR kBq U235 eq 3.22E-01 6.64E-05 1.45E-04 3.22E-01 6.64E-05 1.45E-04 6.22E-06 3.32E-05 6.85E-05 -1.75E-02
ETP-fw CTUe 1.21E+01 1.67E-01 6.62E-03 1.21E+01 1.67E-01 6.62E-03 1.57E-02 8.37E-02 3.19E-03 -2.62E+00
HTP-c CTUh 1.79E-09 3.45E-12 4.51E-13 1.79E-09 3.45E-12 4.51E-13 3.23E-13 1.72E-12 3.77E-13 6.14E-10
HTP-nc CTUh 1E-07 1.87E-10 1.57E-11 1E-07 1.87E-10 1.57E-11 2.02E-11 9.33E-11 1.17E-11 1.1E-07
SQP SQP 1.61E+01 9.99E-02 4.44E-03 1.61E+01 9.99E-02 4.44E-03 9.35E-03 5E-02 2.09E-03 -2.54E-01
PM = Potential incidence of disease due to PM emissions; IR = Potential Human exposure efficiency relative to U235; ETP-fw = Potential comparative
Toxic Unit for ecosystems; HTP-c = Potential comparative Toxic Unit for humans (cancerogenic); HTP-nc = Potential comparative Toxic Unit for humans
(not cancerogenic); SQP = Potential soil quality index
Disclaimer 1 – for the indicator “Potential Human exposure efficiency relative to U235”. This impact category deals mainly with the
eventual impact of low-dose ionizing radiation on human health of the nuclear fuel cycle. It does not consider effects due to possible
nuclear accidents, occupational exposure or radioactive waste disposal in underground facilities. Potential ionizing radiation from the
soil, radon and from some construction materials is also not measured by this indicator.
Disclaimer 2 – for the indicators “abiotic depletion potential for non-fossil resources”, “abiotic depletion potential for fossil resources”,
“water (user) deprivation potential, deprivation-weighted water consumption”, “potential comparative toxic unit for ecosystems”,
“potential comparative toxic unit for humans – cancerogenic”, “Potential comparative toxic unit for humans - not cancerogenic”,
“potential soil quality index”. The results of this environmental impact indicator shall be used with care as the uncertainties on these
results are high as there is limited experience with the indicator.
6. LCA: Interpretation
The most important life cycle phase for cast-in anchor channel influence on resource use, minerals and metals impact
system HTA-CE 40/22P-FV is the manufacturing phase. With category.
regard to the manufacturing phase, the upstream processes of The biogenic global warming potential shows the absorption of
primary and secondary steel along with steel screw and atmospheric carbon dioxide during plant growth in connection
galvanisation dominate all the indicators. Zinc has relevant with packaging (wooden pallets and wooden packaging).
7. Requisite evidence
No evidence required.
8. References
Standards Environmental Product Declarations - Core rules for the product
category of construction products
AC 232
Acceptance Criteria for Anchor Channels in Concrete Elements DIN EN ISO 50001
International Code Council – Evaluation Service (ICC-ES) 2021 Energy management systems - Requirements with guidance for
use ISO 50001:2011
ACI 318
Building Code Requirements for Structural Concrete ACI EN 1992-4
American Concrete Institute 2019 Eurocode 2: Design of concrete structures Part 4: Design of
fastenings for use in concrete 2018
Biocide Products Regulation (BPR)
Regulation (EU) No. 528/2012, European Parliament and EN 13501
Council Dated: 22.05.2012 Fire classification of construction products and building
elements, 2018
Candidate List
Candidate List of substances of very high concern for EOTA TR 047
Authorisation, European Chemicals Agency (ECHA) Technical Report TR 047 Calculation Method for the
performance of Anchor Channels European Organisation for
Construction Products Regulation (CPR) Technical Assessment March 2018
Regulation (EU) No. 305/2011, European Parliament and
Council Dated: 09.03.2011 ETA 09/0339
European Technical Approval ETA-09/0339 Halfen anchor
DIN EN 15804 channel HTA German Institute for Building Technology - DIBt
EN 15804:2012+A2:2019: Sustainability of construction works - Dated: 07.12.2021
7 Environmental Product Declaration - Leviat GmbH - HALFEN mounting and cast-in anchor channel systems
ISO 9001
ETA 19/0438 Quality management systems 2015
European Technical Assessment ETA-19/0438 Halfen hot-rolled
mounting channel HM, special screws German Institute for ISO 15686
Building Technology - DIBt Dated: 12.01.2022 Building and constructed assets - service life planning 2017
ETA 20/1081 MPA NRW
European Technical Assessment ETA-20/1081 Halfen serrated Materialprüfungsamt Nordrhein-Westfalen Dortmund / Germany
anchor channel HZA German Institute for Building Technology -
DIBt Dated: 15.07.2022 Literature
GaBi software
ETA 17/0728 Sphera Solutions GmbH GaBi Software System and Database
European Technical Assessment ETA-17/0728 Halfen anchor for Life Cycle Engineering CUP Version: 2022.2 University of
channel HZA-PS German Institute for Building Technology - Stuttgart Leinfelden Echterdingen
DIBt Dated: 09.12.2022
GaBi documentation
EWC GaBi life cycle inventory data documentation (http://www.gabi-
European Waste Code according to European Waste software.com/international/databases/gabi-data-search/)
Catalogue Directive 2008/98/EC European Parliament and of
the Council 2014 IBU 2021
Institut Bauen und Umwelt e.V.: General Programme
IAS Instructions for the Preparation of EPDs at the Institut Bauen
International Accreditation Service Subsidiary of the und Umwelt e.V., version 2.0., Berlin: Institut Bauen und
International Code Council Brea / California / USA Umwelt e.V., 2021, http://www.ibu-epd.com
ICC ESR 1008 PCR Part A
ICC Evaluation Report 1008 Halfen HTA anchor channels and Calculation Rules for the Life Cycle Assessment and
HS channel bolts International Code Council - Evaluation Requirements on the Project Report,Berlin: Institut Bauen und
Service 2022 Umwelt e.V., www.ibu-epd.com, Version 2.1, 2021
ICC ESR 4016 PCR Part B
ICC Evaluation Report 4016 Halfen HZA anchor channels and Requirements on the EPD for Thin-walled profiles and profiled
HZS channel bolts International Code Council - Evaluation panels, version 1.7, Institut Bauen und Umwelt e.V., www.bau-
Service 2022 umwelt.com, 2019
8 Environmental Product Declaration - Leviat GmbH - HALFEN mounting and cast-in anchor channel systems
Publisher
Institut Bauen und Umwelt e.V. +49 (0)30 3087748- 0
Hegelplatz 1 info@ibu-epd.com
10117 Berlin www.ibu-epd.com
Germany
Programme holder
Institut Bauen und Umwelt e.V. +49 (0)30 3087748- 0
Hegelplatz 1 info@ibu-epd.com
10117 Berlin www.ibu-epd.com
Germany
Author of the Life Cycle Assessment
thinkstep AG +49 711 341817-0
Hauptstrasse 111- 113 info@thinkstep.com
70771 Leinfelden-Echterdingen www.thinkstep.com
Germany
Sphera Solutions GmbH +49 (0)711 341817-0
Hauptstraße 111- 113 info@sphera.com
70771 Leinfelden-Echterdingen www.sphera.com
Germany
Owner of the Declaration
Leviat GmbH +49 2173 970-0
Liebigstrasse 14 info.de@leviat.com
40764 Langenfeld https://www.leviat.com/
Germany
9 Environmental Product Declaration - Leviat GmbH - HALFEN mounting and cast-in anchor channel systems
