ENVIRONMENTAL PRODUCT DECLARATION
as per ISO 14025 and EN 15804+A2
Owner of the Declaration CELO Befestigungssysteme GmbH
Publisher Institut Bauen und Umwelt e.V. (IBU)
Programme holder Institut Bauen und Umwelt e.V. (IBU)
Declaration number EPD-CLO-20240121-CBA1-EN
Issue date 03.04.2024
Valid to 13.09.2028
ResiFIX Pure Epoxy plus EPPSF
CELO Befestigungssysteme GmbH
www.ibu-epd.com | https://epd-online.com
General Information
CELO Befestigungssysteme GmbH ResiFIX Pure Epoxy plus EPPSF
Programme holder Owner of the declaration
IBU – Institut Bauen und Umwelt e.V. CELO Befestigungssysteme GmbH
Hegelplatz 1 Industriestraße 6
10117 Berlin 86551 Aichach
Germany Germany
Declaration number Declared product / declared unit
EPD-CLO-20240121-CBA1-EN The declared product is the two-component reaction resin mortar "ResiFIX
Pure Epoxy plus EPPSF", manufactured by CELO Befestigungssysteme
GmbH. The declared unit is based on 1 kg reaction resin product in the
ratio at which the two components must be mixed before use. The
packaging is also included in the calculation, since the product is sold by
CELO Befestigungssysteme GmbH with its packaging. The declared unit is
indicated in [kg].
This declaration is based on the product category rules: Scope:
Reaction resin products, 01.08.2021 This document covers the two-component reaction resin mortar "ResiFIX
(PCR checked and approved by the SVR) Pure Epoxy plus EPPSF". To prepare the life cycle assessment [LCA],
specific data were collected from the CELO Befestigungssysteme GmbH
manufacturing facility in Plant 2, Germany. The assessment is based on
Issue date data from 2020 which correspond to the yearly average.
The owner of the declaration shall be liable for the underlying information
03.04.2024
and evidence; the IBU shall not be liable with respect to manufacturer
information, life cycle assessment data and evidences.
Valid to
The EPD was created according to the specifications of EN 15804+A2. In
13.09.2028 the following, the standard will be simplified as EN 15804.
Verification
The standard EN 15804 serves as the core PCR
Independent verification of the declaration and data according to ISO
14025:2011
internally X externally
Dipl.-Ing. Hans Peters
(Chairman of Institut Bauen und Umwelt e.V.)
Florian Pronold Angela Schindler,
(Managing Director Institut Bauen und Umwelt e.V.) (Independent verifier)
1 Environmental Product Declaration - CELO Befestigungssysteme GmbH - ResiFIX Pure Epoxy plus EPPSF
Product
+ 5°C 2880 min.
Product description/Product definition + 10°C 1680 min.
The declared product ResiFIX Pure Epoxy plus EPPSF is a + 15°C 1080 min.
two-component reaction resin mortar based on epoxy resin that + 20°C 720 min.
is delivered in a two-component plastic cartridge. The high- + 25°C 540 min.
performance product is applied through a static mixer using a + 35°C 360 min.
manual, battery-operated or pneumatic gun. It was specially + 40°C 240 min.
developed for use in securing threaded rods, rebar or internally
threaded sleeves in concrete. For more information, please refer to the relevant technical data
Marketing of the product in the EU/EFTA (except for sheet.
Switzerland) is governed by Regulation
(EU) No. 305/2011 (CPR). The product requires a Declaration Product performance values in accordance with the Declaration
of Performance subject to ETA-21/0928 and ETA-21/0929 and of Performance with regard to its principal characteristics
CE marking. according to ETA-21/0928 and ETA-21/0929.
Base materials/Ancillary materials
Application The declared product ResiFIX Pure Epoxy plus EPPSF is
The CELO Injection system ResiFIX Pure Epoxy plus is used to delivered as a two-component plastic cartridge and consists of
safely secure threaded rods, internally threaded sleeves and a resin component and a curing agent component in a 3:1
post-mortared rebar connections in cracked and uncracked volume ratio. The mixing ratio between the resin component
C20/25 to C50/60 concrete for a useful life of up to 100 years, and the curing agent component is set automatically as the
and is suitable for installation in hammer-drilled (standard SDS product is pushed out of the cartridge. Curing begins
and hollow bit) and diamond-drilled holes at environmental immediately after the components are mixed.
temperatures between 0°C and 40°C. The CELO Injection
system ResiFIX Pure Epoxy plus has ETA assessments and 1) "This product/article/at least one partial article contains
ICC certifications, including seismic category C1 and C2 for substances in the ECHA candidate list of substances of very
anchoring from M8 to M30 and for rebar connections including high concern (SVHC) (17 January 2023) above a concentration
seismic conditions from 8mm to 40mm, and can be rated for fire of 0.1% by mass: no."
conditions.
2) "This product/article/at least one partial article contains other
Technical Data
CMR substances in categories 1A or 1B which are not on the
The following structural properties are relevant for the declared candidate list, exceeding 0.1 percentage by mass: no"
product ResiFIX Pure Epoxy plus EPPSF as delivered:
Construction Data 3) "Biocide products were added to this construction product or
it has been treated with biocide products (this then concerns a
Name Value Unit
treated product as defined by the (EU) Regulation on Biocidal
Density acc. to DIN 51757 for mixing the two
1.4 g/cm³ Products No. 528/2012): no"
components
Compressive strength acc. to DIN EN 196 Part 1 121.8N/mm² The product considered in this EPD contains individual
Flexural strength acc. to DIN EN 196 Part 1 66 N/mm² components in the following ranges:
Storage:
Resin component:
Store in a cool, dry and dark place; storage temperature: +5°C
Epoxy resin: 40 to 75% by weight
to +35°C
Mineral fillers: 30 to 40% by weight
Other components: < 5% by weight
Shelf life:
24 months in cartridge systems
Curing agent component:
Various polyamines: 40 to 50% by weight
Gel and working time:
Mineral fillers: 30 to 50% by weight
0°C 90 min.
Other components: < 5% by weight
+ 5°C 80 min.
+ 10°C 60 min.
Reference service life
+ 15°C 40 min.
The declared product ResiFIX Pure Epoxy plus EPPSF may be
+ 20°C 30 min.
exposed to a wide range of environmental conditions during the
+ 25°C 12 min.
use phase. Its expected reference service life depends on the
+ 35°C 8 min.
specific installation situation and on the product's resulting
+ 40 °C 8 min.
exposure. The main factors influencing service life are weather
conditions and mechanical and chemical stresses.
Curing time in dry substrate:
0°C 8640 min.
LCA: Calculation rules
product name ResiFIX Pure Epoxy plus EPPSF. The declared
Declared Unit unit is based on 1 kg reaction resin product in the ratio at which
The product declared is a two-component reaction resin mortar the two components must be mixed before use. The mass
manufactured by CELO Befestigungssysteme GmbH with the mixing ratio between the resin component and the curing agent
2 Environmental Product Declaration - CELO Befestigungssysteme GmbH - ResiFIX Pure Epoxy plus EPPSF
component is 4:1 (volume ratio 3:1). The packaging is also Figure 1 Information modules A1 to A3 of the product
included in the calculation at 0.1435 kg per 1 kg of reaction
resin product. The declared unit data are presented in the table
below:
Declared unit data
Name Value Unit
Declared unit 1 kg
System boundary Figure 2 Information modules A1 to A3 of the packaging
Type of EPD: Cradle to factory gate with options. The following
information modules are defined as system boundaries in this Information modules C1 to C4 document
study: deconstruction/demolition for removal from the building,
transport to waste disposal, waste processing and product
Production stage (A1–A3): disposal. Reuse, recovery and recycling potential are
• A1, Raw material extraction, documented in information module D.
• A2, Transport to the manufacturer,
Geographic Representativeness
• A3, Manufacturing.
Land or region, in which the declared product system is
manufactured, used or handled at the end of the product´s
End of life (C1-C4):
lifespan: Germany
• C1, Deconstruction/demolition,
• C2, Transport,
• C3, Waste processing, Comparability
• C4, Disposal. Basically, a comparison or an evaluation of EPD data is only
possible if all the data sets to be compared were created
Reuse, recovery and recycling potential (D) according to EN 15804 and the building context, respectively
the product-specific characteristics of performance, are taken
To precisely determine the indicators and environmental into account.
impacts of the declared unit, a total of 8 information modules The background datasets from the LCA for Experts and
are considered. The information modules A1 to A3 describe the ecoinvent 3.9.1 databases, which this study also draws on, are
material provision, the transport to the production site, as well documented at the following site (Sphera). 2023.1
as the production processes of the product itself. http://www.gabi-software.com/deutsch/index/ (ecoinvent 3.9.1).
http://ecoquery.ecoinvent.org/3.9.1/cutoff/search
The precursor products are sourced from Germany. Transport
is exclusively done by truck. The following process diagrams
illustrate the underlying production process.
LCA: Scenarios and additional technical information
Characteristic product properties of biogenic carbon
No renewable raw materials are used in the product or the
End of Life (C1–C4)
packaging. The biogenic carbon value is therefore reported as
The product is demolished by using an electric chisel. The
zero.
electrical energy consumption for this tool is estimated at 0.05
MJ for the declared unit. The power consumption is calculated
using a European energy mix. Construcion waste is transported
Packaging per declared unit 200 km by truck to a waste treatment facility. At the waste
Name Value Unit treatment facility, the construction waste is shredded and then
Packaging PP 0.1188 kg disposed in a landfill.
Packaging PA6 0.0082 kg
Packaging PE-LD 0.0165 kg
3 Environmental Product Declaration - CELO Befestigungssysteme GmbH - ResiFIX Pure Epoxy plus EPPSF
Name Value Unit The product has no reuse, recovery or recycling potential.
Information module D is therefore declared and reported as
Collected as mixed construction waste 1 kg
zero.
Shredding 1 kg
Name Value Unit
Disposal in landfill 1 kg
Reuse, recovery and recycling potential 0 kg
Reuse, recovery and recycling potential (D), relevant
scenario specifications
4 Environmental Product Declaration - CELO Befestigungssysteme GmbH - ResiFIX Pure Epoxy plus EPPSF
LCA: Results
The results in this calculation refer to the characterisation factors EN 15840+A2/EF 3.1.
DESCRIPTION OF THE SYSTEM BOUNDARY (X = INCLUDED IN LCA; MND = MODULE OR INDICATOR NOT DECLARED; MNR
= MODULE NOT RELEVANT)
Benefits and
Construction loads beyond
Product stage Use stage End of life stage
process stage the system
boundaries
la ire ta m w a Ry lp p u s tro p s n a rT g n iru tc a fu n a M e h t m o rf tro p s n a rTe tis e h t o t e ta g y lb m e s s A e s U e c n a n e tn ia M ria p e R tn e m e c a lp e R tn e m h s ib ru fe R y g re n e la n o ita re p Oe s u re ta w la n o ita re p Oe s u n o itc u rts n o c -e Dn o itilo m e d tro p s n a rT g n is s e c o rp e ts a W la s o p s iD -e s u e R-y re v o c e R-g n ilc y c e Rla itn e to p
A1 A2 A3 A4 A5 B1 B2 B3 B4 B5 B6 B7 C1 C2 C3 C4 D
X X X MND MND MND MND MNR MNR MNR MND MND X X X X X
RESULTS OF THE LCA - ENVIRONMENTAL IMPACT according to EN 15804+A2: 1 kg ResiFIX Pure Epoxy plus EPPSF
Parameter Unit A1-A3 C1 C2 C3 C4 D
Global Warming Potential total (GWP-total) kg CO 2 eq 4.1E+00 4.58E-03 1.75E-02 2.58E-03 1.46E-02 0
Global Warming Potential fossil fuels (GWP-fossil) kg CO 2 eq 3.97E+00 4.53E-03 1.73E-02 2.56E-03 1.46E-02 0
Global Warming Potential biogenic (GWP-biogenic) kg CO 2 eq 1.26E-01 4.91E-05 0 0 0 0
Global Warming Potential luluc (GWP-luluc) kg CO 2 eq 8.91E-04 4.87E-07 1.58E-04 1.92E-05 4.53E-05 0
Depletion potential of the stratospheric ozone layer (ODP) kg CFC11 eq 2.19E-10 8.27E-14 1.49E-15 4.28E-15 3.71E-14 0
Acidification potential of land and water (AP) mol H+ eq 5.13E-03 9.57E-06 6.48E-05 1.34E-05 1.03E-04 0
Eutrophication potential aquatic freshwater (EP-freshwater) kg P eq 2.24E-05 1.67E-08 6.21E-08 8.71E-09 2.93E-08 0
Eutrophication potential aquatic marine (EP-marine) kg N eq 1.76E-03 2.29E-06 3.03E-05 6.13E-06 2.67E-05 0
Eutrophication potential terrestrial (EP-terrestrial) mol N eq 1.89E-02 2.39E-05 3.39E-04 6.77E-05 2.94E-04 0
Formation potential of tropospheric ozone photochemical oxidants kg NMVOC
5.94E-03 6.11E-06 5.84E-05 1.66E-05 8.06E-05 0
(POCP) eq
Abiotic depletion potential for non fossil resources (ADPE) kg Sb eq 2.08E-07 6.95E-10 1.1E-09 2.74E-09 6.72E-10 0
Abiotic depletion potential for fossil resources (ADPF) MJ 8.8E+01 9.43E-02 2.32E-01 5.04E-02 1.94E-01 0
m3 world eq
Water use (WDP) 1.21E-01 9.98E-04 1.96E-04 4.98E-04 1.6E-03 0
deprived
RESULTS OF THE LCA - INDICATORS TO DESCRIBE RESOURCE USE according to EN 15804+A2: 1 kg ResiFIX Pure Epoxy
plus EPPSF
Parameter Unit A1-A3 C1 C2 C3 C4 D
Renewable primary energy as energy carrier (PERE) MJ 8.76E+00 5.64E-02 1.64E-02 4.68E-03 3.16E-02 0
Renewable primary energy resources as material utilization
MJ 0 0 0 0 0 0
(PERM)
Total use of renewable primary energy resources (PERT) MJ 8.76E+00 5.64E-02 1.64E-02 4.68E-03 3.16E-02 0
Non renewable primary energy as energy carrier (PENRE) MJ 6.69E+01 9.43E-02 2.32E-01 5.05E-02 1.94E-01 0
Non renewable primary energy as material utilization (PENRM) MJ 2.11E+01 0 0 0 0 0
Total use of non renewable primary energy resources (PENRT) MJ 8.81E+01 9.43E-02 2.32E-01 5.05E-02 1.94E-01 0
Use of secondary material (SM) kg 0 0 0 0 0 0
Use of renewable secondary fuels (RSF) MJ 0 0 0 0 0 0
Use of non renewable secondary fuels (NRSF) MJ 0 0 0 0 0 0
Use of net fresh water (FW) m3 1.18E-02 4.55E-05 1.81E-05 1.44E-05 4.9E-05 0
RESULTS OF THE LCA – WASTE CATEGORIES AND OUTPUT FLOWS according to EN 15804+A2:
1 kg ResiFIX Pure Epoxy plus EPPSF
Parameter Unit A1-A3 C1 C2 C3 C4 D
Hazardous waste disposed (HWD) kg 7.4E-09 7.38E-12 8.59E-13 1.31E-13 4.23E-12 0
Non hazardous waste disposed (NHWD) kg 6.94E-02 6.91E-05 3.35E-05 1.33E-05 9.71E-01 0
Radioactive waste disposed (RWD) kg 1.31E-03 1.5E-05 3E-07 6.77E-07 2.21E-06 0
Components for re-use (CRU) kg 0 0 0 0 0 0
Materials for recycling (MFR) kg 0 0 0 0 0 0
Materials for energy recovery (MER) kg 0 0 0 0 0 0
Exported electrical energy (EEE) MJ 0 0 0 0 0 0
Exported thermal energy (EET) MJ 0 0 0 0 0 0
RESULTS OF THE LCA – additional impact categories according to EN 15804+A2-optional:
1 kg ResiFIX Pure Epoxy plus EPPSF
Parameter Unit A1-A3 C1 C2 C3 C4 D
Disease
Incidence of disease due to PM emissions (PM) ND ND ND ND ND ND
incidence
Human exposure efficiency relative to U235 (IR) kBq U235 eq ND ND ND ND ND ND
Comparative toxic unit for ecosystems (ETP-fw) CTUe ND ND ND ND ND ND
5 Environmental Product Declaration - CELO Befestigungssysteme GmbH - ResiFIX Pure Epoxy plus EPPSF
Comparative toxic unit for humans (carcinogenic) (HTP-c) CTUh ND ND ND ND ND ND
Comparative toxic unit for humans (noncarcinogenic) (HTP-nc) CTUh ND ND ND ND ND ND
Soil quality index (SQP) SQP ND ND ND ND ND ND
Disclaimer 2 - applies to the following indicators: 'Abiotic shortage potential - non-fossil resources', 'Abiotic shortage potential - fossil
fuels', 'Water deprivation potential (users)', 'Potential comparative toxic unit for ecosystems', 'Potential comparative toxic unit for human
health - carcinogenic effects', 'Potential comparative toxic unit for human health - non-carcinogenic effects', 'Potential soil quality index'.
The results of this environmental impact indicator shall be used with care, as the uncertainties of the results are high and as there is
limited experience with the indicator.
References
DIN 51757 Background database: ecoinvent 3.9.1 Ziirich: ecoinvent (Ed.)
DIN 51757:2011-01 http://www.ecoinvent.org
Testing of mineral oils and related materials - Determination of (26 May 2023)
density.
ETA-21/0928
EN 196 European Technical Assessment
DIN EN 196-1:2016-11
Methods of testing cement - Part 1: Determination of strength. ETA-21/0929
European Technical Assessment
EN 15804 IBU 2021
EN 15804+A2:2019+AC:2021, Sustainability of construction Institut Bauen und Umwelt e.V.: General guidance for the EPD
works - Environmental product declarations - Core rules for the programme of the Institut Bauen und Umwelt e.V., Version 2.0,
product category of construction products. Berlin: Institut Bauen und Umwelt e.V., 2021. www.ibu-epd.com
EN/TR 15941
CEN/TR 15941:2010-03: Sustainability of construction works - PCR Part A
Environmental product declarations - Methodology for selection Product Category Rules for Building-Related Products and
and use of generic data Services - Calculation Rules for Life Cycle Assessment and
Requierements on the Project Report V1.3, Institut Bauen und
ISO 14025 Umwelt e.V., 08.2022
DIN EN ISO 14025:2011-10, Environmental labels and
declarations - Type III PCR: Reaction resin products
environmental declarations - Principles and procedures. Guidance-Texts for Building-Related Products and Services-
PART B: Requirements on the Environmental Product
ISO 14044 Declarations for Reaction Resin Products,1 August 2021
DIN EN ISO 14044:2006-10, Environmental management - Life
cycle assessment - Requirements and guidelines. Sphera
LCA for Experts: 2023.1
Further references Leinfelden-Echterdingen; Sphera
Solution GmbH (Ed.)
ECHA candidates list http://www. gabi-software.com/deutsch/index/
https://echa.europa.eu/de/candiate-list-substances-in-articles (26 May 2023)
ECHA list Regulation (EU) No. 305/2011 (CPR)
https://echa.europa.eu/de/candiate-list-table
Regulation (EU) No. 528/2012 (Biocidal Products Regulation)
ecoinvent 3.9.1
6 Environmental Product Declaration - CELO Befestigungssysteme GmbH - ResiFIX Pure Epoxy plus EPPSF
Publisher
Institut Bauen und Umwelt e.V. +49 (0)30 3087748- 0
Hegelplatz 1 info@ibu-epd.com
10117 Berlin www.ibu-epd.com
Germany
Programme holder
Institut Bauen und Umwelt e.V. +49 (0)30 3087748- 0
Hegelplatz 1 info@ibu-epd.com
10117 Berlin www.ibu-epd.com
Germany
Author of the Life Cycle Assessment
FIT-Umwelttechnik GmbH 05362 72 69 474
Westerstr. 13 bertram@fit-umwelttechnik.de
38442 Wolfsburg www.fit-umwelttechnik.com
Germany
Owner of the Declaration
CELO Befestigungssysteme GmbH +49 08251 904850
Industriestraße 6 info@celofixings.de
86551 Aichach www.celofixings.de
Germany
7 Environmental Product Declaration - CELO Befestigungssysteme GmbH - ResiFIX Pure Epoxy plus EPPSF
