ENVIRONMENTAL PRODUCT DECLARATION
as per ISO 14025 and EN 15804+A2
Owner of the Declaration Etex Building Performance International
Programme holder Institut Bauen und Umwelt e.V. (IBU)
Publisher Institut Bauen und Umwelt e.V. (IBU)
Declaration number EPD-ETE-20200285-IBC1-EN
Issue date 01.04.2021
Valid to 31.03.2026
Duripanel B1
Etex Germany Exteriors GmbH
www.ibu-epd.com | https://epd-online.com
Umwelt Produktdeklaration Name des Herstellers – Name des Produkts
1. General Information
Etex Germany Exteriors GmbH Duripanel B1
Programme holder Owner of the declaration
IBU – Institut Bauen und Umwelt e.V. Etex Building Performance International
Panoramastr. 1 500 rue Marcel Demonque
10178 Berlin 84915 Avignon Cedex 9
Germany FRANCE
Declaration number Declared product / declared unit
EPD-ETE-20200285-IBC1-EN 1m² Duripanel B1 with thickness 18mm.
This declaration is based on the product Scope:
category rules:
Wood cement - Mineral-bonded wooden composites, The life cycle assessment is based on production data
01.2019 of Duripanel B1 of the year 2018 at the production site
(PCR checked and approved by the SVR) of Etex Germany Exteriors GmbH in Beckum,
Germany.
Issue date The results of the life cycle assessment provided in this
01.04.2021 EPD are based on a thickness of 18mm and are
globally valid.
Valid to The LCA results for additional thicknesses are
declared in an annexe to this EPD.
31.03.2026
The owner of the declaration shall be liable for the
underlying information and evidence; the IBU shall not
be liable with respect to manufacturer information, life
cycle assessment data and evidences.
The EPD was created according to the specifications
of EN 15804+A2. In the following, the standard will be
simplified as EN 15804.
Verification
The standard EN 15804 serves as the core PCR
Independent verification of the declaration and data
according to ISO 14025:2010
Dipl. Ing. Hans Peters internally x externally
(chairman of Institut Bauen und Umwelt e.V.)
Dr. Alexander Röder Mr Carl-Otto Neven
(Managing Director Institut Bauen und Umwelt e.V.)) (Independent verifier)
2. Product
2.1 Information about the enterprise
Etex is an international building materials specialist For the placing on the market of the product in the
with headquarters in Belgium since 1905. The Etex European Union/European Free Trade Association
group operates 101 production sites in 42 countries (EU/EFTA) (with the exception of Switzerland)
and employs over 13 200 people worldwide. Regulation (EU) No. 305/2011 (CPR) applies. The
Duripanel is produced at the production site of Etex construction product is covered by the harmonized
Germany Exteriors GmbH. declaration of performance No. Si-
DOP/Duripanel_B1/v01.10.2020 taking into
2.2 Product description/Product definition consideration EN 13986: 2015, Wood-based panels for
Duripanel B1 is a three-layer cement-bonded use in construction - Characteristics, evaluation of
particleboard according to EN 634-1 and -2 for internal conformity and marking and the CE-marking.
and external construction applications. It mainly For the application and use the respective national
consists of the natural raw material wood particles and provisions apply.
cement.
It is being produced in different thicknesses between 8 2.3 Application
and 40 mm. It is available in an unsanded smooth or The Duripanel B1 base panel with straight edges can
sanded surface, with smooth trimmed edges or with be used in timber frame construction, high-quality
tongue and groove. The surface colour is mainly being interior finishing and container construction as a load-
characterized by the fine wood particles in the outside bearing and stiffening wood-based panel.
layers.
2 Environmental Product Declaration Etex Germany Exteriors GmbH – Duripanel B1
The Duripanel B1 installation panels with tongue and This article contains substances listed in the candidate
groove can be used for supporting formwork and dry list (date: 19.01.2021) exceeding 0.1 percentage by
subfloors with high compressive strength. mass: no.
This article contains other carcinogenic, mutagenic,
2.4 Technical Data reprotoxic (CMR) substances in categories 1A or 1B
which are not on the candidate list, exceeding 0.1
The constructional data shown in the table are valid for percentage by mass: no.
all thicknesses and surfaces (sanded/unsanded), Biocide products were added to this construction
unless where indicated otherwise. product or it has been treated with biocide products
(this then concerns a treated product as defined by the
Constructional data (EU) Ordinance on Biocide Products No. 528/2012):
Name Value Unit no.
Raw density acc. to EN 634-
≥ 1000 kg/m³
2:2007; EN 13986:2004+A1:2015 2.7 Manufacture
Grammage (18 mm) 22.7 kg/m2 The production of large-format panels from wood
Bending strength (longitudinal) ≥ 9 N/mm2 cement takes place according to a largely automated,
Bending strength (transverse) ≥ 9 N/mm2 semi-dry spreading process in which no excess water
E-module (longitudinal) ≥ 4500 N/mm2 is produced. In a mechanical mixer, the litter mixture of
E-module (transverse) ≥ 4500 N/mm2 wood chips, cement, recycled material from trimming
Tensile strength rectangular waste, auxiliary materials and water is processed. The
(internal bond) ≥ 0.5 N/mm2 material is evenly distributed on carrier plates via a
mechanical throw sifting system. Excess material at
Thermal conductivity λ acc. to DIN
0.23 W/(mK) the edges is returned directly to the spreader. The
EN 13986:2015
scattered material is pressed, stored in a climatic
Water vapour diffusion resistance
40 (moist); chamber for setting (heat exchanger, steam generation
factor µ acc. to DIN EN ISO -
67 (dry) via natural gas), the hardened sheets restacked,
12572:2001
trimmed and temporarily stored for 28 days. The
Moisture content at 23 °C, 80%
9 Vol. % panels are then dried in a circulating air oven to the
acc. to DIN EN ISO 12571:2000
moisture content required for delivery.
Coefficient of thermal expansion
11 10-6K-1
αt
The quality management system of the company and
Swelling in thickness 24h acc. to
≤ 1,5 % the production facility are certified according to ISO
EN 634-2: 2007
9001:2015.
Sound absorption coefficient (only 10 at 250-
with reference to the 500Hz / 30
% 2.8 Environment and health during
corresponding component design) at 1000-
manufacturing
acc. to EN 13986:2004+A1:2015 2000Hz
During the entire manufacturing process, no health and
safety measures are required beyond the legally
stipulated occupational health and safety measures for
For more detailed info on product characteristics
commercial enterprises.
please refer to the latest DOP.
Air: Any dust produced is collected in filter systems
The performance data of the product is in accordance
and partially recycled. The emissions are well below
with the declaration of performance with respect to its
the limit values of TA Luft.
essential characteristics according to the standards
mentioned in the headline in the table for
Water/Soil: The water resulting from production and
constructional data.
plant cleaning is mechanically clarified in wastewater
treatment plants on the factory premises and reused in
the production process.
2.5 Delivery status
Duripanel B1 basic panels are available in two sizes
Noise: Noise emissions from production plants to the
1250 x 2600 mm or 1250 x 3100 mm.
environment are below the permissible limits.
The panels are delivered sanded and unsanded in
various thicknesses:
The environmental management system of the
8, 10, 12, 14, 16, 18, 20, 22, 24, 28, 32, 36, 40 mm.
company and the production facility are certified ISO
14001:2015.
Duripanel B1 installation panels are available in sizes
1250 x 625 mm. The panels are delivered sanded on
2.9 Product processing/Installation
both sides in thicknesses 18 and 25 mm.
The processing of Duripanel can include the following
processes, for example: sawing, drilling, grinding.
2.6 Base materials/Ancillary materials
Under certain conditions Duripanel can be milled.
The main raw materials used are (in weight
percentages; dry) :
Fixing the boards will require appropriate means,
- 55-75% Portland cement
which will depend upon the application and bearing
- 15-25% spruce wood (Atro)
structure. Boards can be installed using screws or
- 5-15% recycled production residues
glues. Under certain conditions, the boards can be
fixed using clamps.
By using cement as a binder, no binder related
When selecting structurally necessary additional
isocyanates, synthetic resin or formaldehyde are being
products, care must be taken that these do not
added. No wood protection agents are being used.
adversely affect the described properties of the
3 Environmental Product Declaration Etex Germany Exteriors GmbH – Duripanel B1
environmental compatibility of the construction
products mentioned.
2.14 Extraordinary effects
The local regulations for the workers’ health and safety
and the environment apply (e.g. trade associations or Fire
ordinance on hazardous substances). Also, when The Duripanel B1 boards have a fire classification
processing the above-mentioned products, the usual according to EN 13501-1 as given in the table below.
occupational health and safety measures must be
observed in accordance with the manufacturer's Fire protection
instructions. It should be noted that dust produced Name Value
during processing can react alkaline (pH value: approx. Building material class - base panel B
12). The machining tools and equipment used at the Smoke gas development - base panel s1
workplace should be such that the relevant dust limits Burning droplets - base panel d0
are observed. Building material class - installation panel Bfl
For example, in Germany the general dust limit value Smoke gas development - installation panel s1
is given in the directive TRGS 900. According to Burning droplets - installlation panel -
current knowledge, water, air and soil cannot be
endangered if wood cement is processed as intended. Water
No ingredients that could be hazardous to water are
2.10 Packaging washed out (see also item Evidence: Eluate analysis).
PE shrink films, paper, wooden pallets and steel The pH value is basic (pH ≥ 12).
strapping are used as packaging materials. The
wooden pallets used are one-way pallets. Mechanical destruction
Extraordinary effects related to a mechanical
destruction (e.g. emissions) are not known.
2.11 Condition of use
Duripanel building boards are resistant to the effects of 2.15 Re-use phase
moisture and are not physically affected when used in Several possibilities exist for the boards after the end-
humid or wet conditions. Some performance of-life of the application in which they were used.
characteristics are affected by moisture content. The
panels do not promote mould growth and are resistant In undamaged form, the dismantled products can be
to attacks by insects or vermin. used again in accordance with their original purpose
or, for example, be reused as foundation wall
Setting (hydration) of the cement-water mixture protection.
produces hardened cement paste (calcium silicate If not contaminated with other building construction
hydrates) with embedded wood chips, ground material, the boards can be ground up again and
production waste and auxiliary materials, with the reused as an additive in the production of wood
proportions indicated in the item 2.5 "Base materials". cement (material recycling).
Over the period of use, free lime from the cement
reacts with carbon dioxide from the air to form calcium Furthermore, the products referred to could be used as
carbonate (carbonation). filler and bulk material in civil engineering, road
construction or e.g. for noise barriers (material
Wood cement contains approx. 9-11 % water recycling).
(equilibrium moisture) which can vary with the
environmental conditions. In addition, material and energetic recycling in the
cement plant is possible.
2.12 Environment and health during use
Duripanel B1 is chemically inert. When the product is 2.16 Disposal
used as designed, the current state of knowledge For the consideration of possible disposal channels,
indicates that hazards to water, air and soil cannot the following disposal stages are proposed:
arise.
A) Production waste (before use)
The ingredients of the construction product are firmly B) Waste generated before use
bound in the state of use. Dust emissions will not occur a) at a finishing company that cuts panels to size
unless the boards are machined with abrasive tools. In b) during installation on the building site
case of contact (skin, eye, mouth contact), it should be C) Waste after use, when a building is demolished or
noted that hardened cement paste reacts slightly when structural changes are made during the use
alkaline in combination with moisture. phase of the building.
2.13 Reference service life Disposal channels at stage A)
The service life according to the “Bundesinstitut für If the wood cement products are separated by type in
Bau-, Stadt- und Raumforschung“ (BBSR) table the factory, they can be ground again and reused as
“Service lives of components for life cycle assessment an additive in the production of wood cement (material
according to Bewertungssystem Nachhaltiges recycling). This shall be preferred.
Bauen (BNB)" is indicated to be >50 years. Thermal treatment in residual waste treatment plants
Over the service life, free lime in the cement reacts and cement works can be considered.
with carbon dioxide in the air to form calcium The lowest priority route may be landfill.
carbonate (carbonation). There will be no verifiable
influences on ageing when the products are applied in Disposal channels at stage B) and C)
accordance with the generally accepted rules of
technology.
4 Environmental Product Declaration Etex Germany Exteriors GmbH – Duripanel B1
a) At collection: keeping cement-bonded particleboard
separate from wood waste as well as from other The following waste codes are suggested:
mineral wastes Disposal channel A) 10 13 11 (wastes from cement-
b) Thermal treatment and/or energy recovery based composite materials other than those mentioned
c) Landfill in 10 13 09 and 10 13 10).
Disposal channels B) and C) 17 09 04 (mixed
As for disposal facilities, depending on the composition construction and demolition wastes other than those
and quantity of waste, thermal residual waste mentioned in 17 09 01, 17 09 02 and 17 09 03).
treatment plants and cement works can be considered.
As the landfill classes are being defined differently in 2.17 Further information
the member states, the landfill class of the respective Further information can be found on the homepage
country applies. https://www.siniat.com/.
3. LCA: Calculation rules
3.1 Declared Unit requirement. These modules are defined on
The functional unit declared in this EPD is 1m² of building level in general.
Duripanel B1 with a thickness of 18mm (abbreviated
as 1m²18mm).
End-of-life stage (C1-C4):
In an annexe to this EPD, the LCA results for the other
Two end-of-life scenarios were considered:
existing thicknesses are declared.
1) Scenario 1: 100% recycling in cement plant.
Declared unit
Due to the wood content of Duripanel B1, the shredded
Name Value Unit
product can reduce the use of energy in the cement
Declared unit 1 m²
plant during cement clinker production.
Gross density used in calculations
1263 kg/m3 Simultaneously, the other raw material components in
based on 2018 average data
the wood cement boards help to reduce the use of
Grammage 22.7 kg/m2
virgin raw materials in the cement plant. Energy and
Conversion factor to 1 kg (kg/m²) 22.7 -
material credits were assigned using the substitution
Layer thickness 0,018 m
approach. The resulting credits from energy recovery
and material recycling are assigned to module D.
2) Scenario 2: 100% landfilling.
3.2 System boundary
Type of the EPD: cradle to grave.
For both scenarios, the following processes were
The following life cycle stages and modules are
included:
included:
 energy consumption for deconstruction and
demolition
Production stage (A1-A3):
 manufacturing of pre products and  transportation to disposal
transportation to the manufacturing site  waste processing and recycling or landfilling
 energy consumption during production of product
 recycling and disposal of production wastes
 production of packaging Loads and benefits beyond system boundary (D):
 loads and benefits from recycling/landfilling of
production waste, packaging, installation
Construction stage (A4-A5):
losses and product waste.
 transportation of product to the construction
site
 energy consumption during the installation of
products
3.3 Estimates and assumptions
 production of fixing material
Most of the input and output influences of the Life
 disposal of installation wastes including Cycle Inventory Analyses could be depicted using
emissions of biogenic CO2 from the wood corresponding data from the GaBi database.
content There were no data records available for the wooden
 incineration/recycling of packaging materials pallets, they were approximated using the solid
construction timber dataset. For well water, a worst
(potential benefits from energy substitution
case scenario dataset “tap water from groundwater”
within the incineration process are declared in
was used. For the Duripanel product waste sent to
module D) including emissions of biogenic landfill, a combination of an inert waste dataset and a
CO2 from renewable packaging materials municipal solid waste dataset was used in a ratio to
match the calorific value of the Duripanel B1 waste.
Bluewater consumption is taken into consideration in
Use stage (B1-B7):
the background data system. Water which is
 efforts for the use of the product,
embedded in the product, as well as water which is
maintenance and operational efforts
evaporated from the product during production, is
 modules B3, B4, B5 are declared as MNR included in the calculations.
(module not relevant) according to the IBU
5 Environmental Product Declaration Etex Germany Exteriors GmbH – Duripanel B1
3.4 Cut-off criteria Allocation of upstream data
All available data from production processes were The product receives recycled water provided by
considered, i.e., all pre-products used, thermal energy another production line.
and electric power consumption as well as waste Allocation in foreground data
management processes using the best available life The production process does not deliver any co-
cycle inventory (LCI) datasets. This includes input products. In module A1-A3, specific raw material,
flows with a contribution of less than 1% of mass or water and transport data were available.
energy. Thermal energy used at plant level in a cogeneration
Production of capital equipment, facilities and unit could not be directly allocated to the product and
infrastructure required for manufacture are outside the was allocated via recalculation based on consumed
scope of this assessment. amounts of electricity and steam.
Allocation for waste materials
3.5 Background data The environmental burden of waste treatment of the
The GaBi ts software was used to model the product installation loss and the incineration of packaging is
life cycle. The background data were sourced from the assigned to the system in A5. The resulting credits for
GaBi database. thermal and electrical energy are declared in module
D.
3.6 Data quality The environmental burdens of the product at end-of-life
This study is mainly based on primary data collected scenarios are assigned to C3 and C4, the resulting
directly from the manufacturing site and therefore data credits for thermal and electrical energy are declared in
quality can be assumed to be very good. module D.
Background data are from the GaBi database, last
update was in 2020. 3.9 Comparability
Basically, a comparison or an evaluation of EPD data
3.7 Period under review is only possible if all the data sets to be compared
Data for the entire production period of 2018 were were created according to EN 15804 and the building
collected and used for this EPD. context, respectively the product-specific
characteristics of performance, are taken into account.
3.8 Allocation
Allocation in background data GaBi database version 2020.1, SP40 serves as
Specific information on allocation within the background database for the calculation of the life
background data is given in the GaBi documentation. cycle assessment. .
4. LCA: Scenarios and additional technical information
Characteristic product properties Use or application of the installed product (B1) see
Information on biogenic Carbon section 2.12 "Use"
No efforts and releases of substances occur during the
normal (i.e. anticipated) use phase
Information on describing the biogenic Carbon Name Value Unit
Content at factory gate
Name Value Unit Maintenance (B2)
Biogenic Carbon Content in No efforts occur during maintenance.
2.22 kg C
product Name Value Unit
Biogenic Carbon Content in Water consumption 0 m3
0.19 kg C
accompanying packaging Auxiliary 0 kg
Other resources 0 kg
Electricity consumption 0 kWh
Other energy carriers 0 MJ
Material loss 0 kg
Transport to the building site (A4)
Name Value Unit
Transport distance 300 km
Capacity utilisation (including empty
61 %
runs)
Gross density of products transported 1263 kg/m3
Installation into the building (A5)
Name Value Unit
Auxiliary galvanized steel screws 0.12 kg
Electricity consumption 0.075 kWh
Material loss 2.27 kg
Dust in the air 0 kg
VOC in the air 0 kg
6 Environmental Product Declaration Etex Germany Exteriors GmbH – Duripanel B1
Reference service life
Name Value Unit
Reference service life (according
- a
to ISO 15686-1, -2, -7 and -8)
Life Span (according to BBSR) >=50 a
Life Span according to the
- a
manufacturer
Declared product properties (at
- -
the gate) and finishes
Design application parameters (if
instructed by the manufacturer),
including the references to the - -
appropriate practices and
application codes
An assumed quality of work, when
installed in accordance with the - -
manufacturer’s instructions
Outdoor environment, (for outdoor
applications), e.g. weathering,
pollutants, UV and wind exposure, - -
building orientation, shading,
temperature
Indoor environment (for indoor
applications), e.g. temperature, - -
moisture, chemical exposure
Usage conditions, e.g. frequency
- -
of use, mechanical exposure
Maintenance e.g. required
frequency, type and quality and - -
replacement of components
Operational energy use (B6) and Operational water
use (B7)
No efforts occur in modules B6 and B7.
Name Value Unit
Water consumption 0 m3
Electricity consumption 0 kWh
Other energy carriers 0 MJ
Equipment output 0 kW
End-of-life (C1-C4)
Two end-of-life scenarios are considered :
- scenario 1: 100% recycling in cement plant
- scenario 2: 100% landfill
Name Value Unit
Collected as mixed construction
22.82 kg
waste
Recycling (scenario 1) 22.82 kg
Recycling (scenario 2) 0.12 kg
Landfilling (scenario 1) 0 kg
Landfilling (scenario 2) 22.7 kg
Reuse, recovery and/or recycling potentials (D),
relevant scenario information
Possible benefits from the recycling of production
waste and installation losses were considered. Also,
benefits from the incineration of packaging were
considered. Additionally, benefits from the recycling of
the product at the end-of-life was taken into account
according to the selected scenario.
Name Value Unit
Recycled production waste 1.25 kg
Recycled installation losses 0.796 kg
PE packaging 11 g
Wood packaging 472 g
Paper packaging 0.75 g
Steel strip packaging 5 g
EoL Recycling (scenario 1) 22.8 kg
EoL Recycling (scenario 2) 0.12 kg
7 Environmental Product Declaration Etex Germany Exteriors GmbH – Duripanel B1
5. LCA: Results
Disclaimer – for the indicator EF-freshwater, this indicator (the kg PO4 eq.) has been calculated as “kg P eq.” as
required in the characterization model EC-JRC : EF 3.0; http://eplca.jrc.ec.europa.eu/LCDN/developerEF.xhtml.
The characterization factors are available both in ILCD structure and as Excel file and they are identified by the
name EN_15804.
DESCRIPTION OF THE SYSTEM BOUNDARY (X = INCLUDED IN LCA; ND = MODULE OR INDICATOR NOT
DECLARED; MNR = MODULE NOT RELEVANT)
BENEFITS AND
CONSTRUCTI LOADS
PRODUCT STAGE ON PROCESS USE STAGE END OF LIFE STAGE BEYOND THE
STAGE SYSTEM
BOUNDARIES
8 Environmental Product Declaration Etex Germany Exteriors GmbH – Duripanel B1
lairetam
waR
ylppus tropsnarT
gnirutcafunaM
eht
morf
tropsnarT
etis
eht
ot
etag
ylbmessA esU
ecnanetniaM
riapeR
tnemecalpeR tnemhsibrufeR
ygrene
lanoitarepO esu
retaw
lanoitarepO esu
noitcurtsnoc-eD
noitilomed tropsnarT
gnissecorp
etsaW
lasopsiD -esueR -yrevoceR -gnilcyceR laitnetop
A1 A2 A3 A4 A5 B1 B2 B3 B4 B5 B6 B7 C1 C2 C3 C4 D
X X X X X X X MNR MNR MNR X X X X X X X
RESULTS OF THE LCA - ENVIRONMENTAL IMPACT according to EN 15804+A2: 1 m²18mm Duripanel B1
Core Indicator Unit A1-A3 A4 A5 B1 B2 B6 B7 C1 C2 C3/1 C3/2 C4/1 C4/2 D/1 D/2
- -
8.97E+ 3.04E+ 0.00E+ 0.00E+ 0.00E+ 0.00E+ 1.28E+ 0.00E+ 0.00E+ 8.90E+
GWP-total [kg CO2-Eq.]
0
5.33E-1
0 0 0 0 0
3.03E-28.71E-2
0 0 0 0
6.41E+ 1.07E+
0 0
- -
1.83E+ 2.35E+ 0.00E+ 0.00E+ 0.00E+ 0.00E+ 1.27E+ 0.00E+ 0.00E+ 1.15E+
GWP-fossil [kg CO2-Eq.]
1
5.30E-1
0 0 0 0 0
3.02E-28.66E-2
0 0 0 0
6.40E+ 1.06E+
0 0
-
-8.89E- 0.00E+ 0.00E+ 0.00E+ 0.00E+ -1.45E- 0.00E+ 0.00E+ 7.74E+ -6.75E- -1.98E-
GWP-biogenic [kg CO2-Eq.] 9.34E+
4
6.88E-1
0 0 0 0
1.01E-4
4
4.24E-3
0 0 0 3 3
0
0.00E+ 0.00E+ 0.00E+ 0.00E+ 0.00E+ 0.00E+ -8.46E- -6.68E-
GWP-luluc [kg CO2-Eq.] 6.33E-34.29E-31.06E-3
0 0 0 0
4.38E-57.01E-41.84E-3
0 0
1.05E-3
4 4
4.96E- 9.72E- 8.26E- 0.00E+ 0.00E+ 0.00E+ 0.00E+ 6.64E- 1.59E- 2.80E- 0.00E+ 0.00E+ 1.83E- -4.36E- -8.91E-
ODP [kg CFC11-Eq.]
14 17 15 0 0 0 0 16 17 14 0 0 15 15 15
0.00E+ 0.00E+ 0.00E+ 0.00E+ 0.00E+ 0.00E+ -5.48E- -1.76E-
AP [mol H+-Eq.] 2.14E-26.12E-43.58E-3 6.66E-51.00E-42.81E-3 3.86E-3
0 0 0 0 0 0 3 3
0.00E+ 0.00E+ 0.00E+ 0.00E+ 0.00E+ 0.00E+ -1.41E- -1.25E-
EP-freshwater [kg PO4-Eq.] 3.25E-51.61E-62.08E-5
0 0 0 0
8.06E-82.64E-73.40E-6
0 0
1.67E-4
6 6
0.00E+ 0.00E+ 0.00E+ 0.00E+ 0.00E+ 0.00E+ -1.95E- -4.38E-
EP-marine [kg N-Eq.] 7.24E-31.88E-41.20E-3 1.48E-53.07E-56.23E-4 2.31E-3
0 0 0 0 0 0 3 4
0.00E+ 0.00E+ 0.00E+ 0.00E+ 0.00E+ 0.00E+ -2.15E- -4.71E-
EP-terrestrial [mol N-Eq.] 7.81E-22.23E-31.19E-2 1.56E-43.65E-46.55E-3 1.26E-2
0 0 0 0 0 0 2 3
0.00E+ 0.00E+ 0.00E+ 0.00E+ 0.00E+ 0.00E+ -5.95E- -1.29E-
POCP [kg NMVOC-Eq.]2.21E-25.07E-43.56E-3 4.06E-58.29E-51.71E-3 5.81E-3
0 0 0 0 0 0 3 3
0.00E+ 0.00E+ 0.00E+ 0.00E+ 0.00E+ 0.00E+ -3.76E- -1.49E-
ADPE [kg Sb-Eq.] 8.33E-74.28E-82.19E-5 8.74E-97.00E-93.68E-7 5.02E-8
0 0 0 0 0 0 7 7
- -
1.11E+ 7.06E+ 1.59E+ 0.00E+ 0.00E+ 0.00E+ 0.00E+ 1.15E+ 2.23E+ 0.00E+ 0.00E+ 9.31E+
ADPF [MJ] 5.31E-1 1.03E+ 1.64E+
2 0 1 0 0 0 0 0 1 0 0 0
2 1
[m³ world-Eq 0.00E+ 0.00E+ 0.00E+ 0.00E+ 0.00E+ 0.00E+ -4.10E- -9.23E-
WDP 2.72E-15.16E-31.37E-1 6.58E-38.44E-42.77E-1 5.25E-2
deprived] 0 0 0 0 0 0 2 2
GWP = Global warming potential; ODP = Depletion potential of the stratospheric ozone layer; AP = Acidification potential of land and water; EP =
Caption Eutrophication potential; POCP = Formation potential of tropospheric ozone photochemical oxidants; ADPE = Abiotic depletion potential for non-
fossil resources; ADPF = Abiotic depletion potential for fossil resources; WDP = Water (user) deprivation potential
RESULTS OF THE LCA - INDICATORS TO DESCRIBE RESOURCE USE according to EN 15804+A2: 1
m²18mm Duripanel B1
Indicator Unit A1-A3 A4 A5 B1 B2 B6 B7 C1 C2 C3/1 C3/2 C4/1 C4/2 D/1 D/2
PERE [MJ] 3.36E+1 4.08E-1 2.04E+10.00E+00.00E+00.00E+00.00E+0 2.35E-1 6.68E-2 9.01E+10.00E+00.00E+08.11E+1-1.71E+0-3.29E+0
PERM [MJ] 8.75E+10.00E+0-7.30E+00.00E+00.00E+00.00E+00.00E+00.00E+00.00E+0-8.02E+10.00E+00.00E+0-8.02E+10.00E+00.00E+0
PERT [MJ] 1.21E+2 4.08E-1 1.31E+10.00E+00.00E+00.00E+00.00E+0 2.35E-1 6.68E-2 9.90E+00.00E+00.00E+0 8.32E-1-1.71E+0-3.29E+0
PENRE [MJ] 1.10E+27.09E+01.63E+10.00E+00.00E+00.00E+00.00E+0 5.31E-1 1.16E+02.23E+10.00E+00.00E+09.31E+0-1.03E+2-1.64E+1
PENRM [MJ] 4.40E-1 0.00E+0-4.40E-10.00E+00.00E+00.00E+00.00E+00.00E+00.00E+00.00E+00.00E+00.00E+00.00E+00.00E+00.00E+0
PENRT [MJ] 1.11E+27.09E+01.59E+10.00E+00.00E+00.00E+00.00E+0 5.31E-1 1.16E+02.23E+10.00E+00.00E+09.31E+0-1.03E+2-1.64E+1
SM [kg] 1.49E+00.00E+0 1.49E-1 0.00E+00.00E+00.00E+00.00E+00.00E+00.00E+00.00E+00.00E+00.00E+00.00E+00.00E+00.00E+0
RSF [MJ] 0.00E+00.00E+00.00E+00.00E+00.00E+00.00E+00.00E+00.00E+00.00E+00.00E+00.00E+00.00E+00.00E+00.00E+00.00E+0
NRSF [MJ] 0.00E+00.00E+00.00E+00.00E+00.00E+00.00E+00.00E+00.00E+00.00E+00.00E+00.00E+00.00E+00.00E+00.00E+00.00E+0
FW [m³] 1.35E-2 4.76E-4 4.69E-3 0.00E+00.00E+00.00E+00.00E+0 2.72E-4 7.78E-5 1.15E-2 0.00E+00.00E+0 1.61E-3-2.15E-3-4.07E-3
PERE = Use of renewable primary energy excluding renewable primary energy resources used as raw materials; PERM = Use of
renewable primary energy resources used as raw materials; PERT = Total use of renewable primary energy resources; PENRE = Use of
non-renewable primary energy excluding non-renewable primary energy resources used as raw materials; PENRM = Use of non-
Caption
renewable primary energy resources used as raw materials; PENRT = Total use of non-renewable primary energy resources; SM = Use
of secondary material; RSF = Use of renewable secondary fuels; NRSF = Use of non-renewable secondary fuels; FW = Use of net fresh
water
RESULTS OF THE LCA – WASTE CATEGORIES AND OUTPUT FLOWS according to EN 15804+A2:
1 m²18mm Duripanel B1
Indicator Unit A1-A3 A4 A5 B1 B2 B6 B7 C1 C2 C3/1 C3/2 C4/1 C4/2 D/1 D/2
HWD [kg] 3.24E-7 3.28E-7 4.24E-8 0.00E+00.00E+00.00E+00.00E+02.20E-105.36E-8 9.25E-9 0.00E+00.00E+0 7.16E-8-6.07E-8-8.29E-9
NHWD [kg] 3.29E+0 1.12E-3 2.46E+00.00E+00.00E+00.00E+00.00E+0 3.77E-4 1.84E-4 1.59E-2 0.00E+00.00E+02.12E+1-2.71E-2-9.58E-3
RWD [kg] 1.58E-3 1.31E-5 3.67E-4 0.00E+00.00E+00.00E+00.00E+0 8.06E-5 2.14E-6 3.39E-3 0.00E+00.00E+0 1.09E-4-4.99E-4-1.14E-3
CRU [kg] 0.00E+00.00E+00.00E+00.00E+00.00E+00.00E+00.00E+00.00E+00.00E+00.00E+00.00E+00.00E+00.00E+00.00E+00.00E+0
MFR [kg] 8.81E-1 0.00E+0 9.31E-2 0.00E+00.00E+00.00E+00.00E+00.00E+00.00E+01.62E+1 9.98E-2 0.00E+00.00E+00.00E+00.00E+0
MER [kg] 3.65E-1 0.00E+0 3.65E-2 0.00E+00.00E+00.00E+00.00E+00.00E+00.00E+06.66E+00.00E+00.00E+02.36E+00.00E+00.00E+0
EEE [MJ] 2.20E-3 0.00E+01.54E+00.00E+00.00E+00.00E+00.00E+00.00E+00.00E+00.00E+00.00E+00.00E+00.00E+00.00E+00.00E+0
EET [MJ] 5.07E-3 0.00E+02.37E+00.00E+00.00E+00.00E+00.00E+00.00E+00.00E+00.00E+00.00E+00.00E+00.00E+00.00E+00.00E+0
HWD = Hazardous waste disposed; NHWD = Non-hazardous waste disposed; RWD = Radioactive waste disposed; CRU = Components
Caption for re-use; MFR = Materials for recycling; MER = Materials for energy recovery; EEE = Exported electrical energy; EEE = Exported
thermal energy
RESULTS OF THE LCA – additional impact categories according to EN 15804+A2-optional:
1 m²18mm Duripanel B1
Indicator Unit A1-A3 A4 A5 B1 B2 B6 B7 C1 C2 C3/1 C3/2 C4/1 C4/2 D/1 D/2
[Disease 5.59E- 6.63E-
PM 4.52E-7 4.06E-9 6.05E-80.00E+00.00E+00.00E+00.00E+0 2.35E-80.00E+00.00E+04.25E-8-1.85E-7-2.36E-8
Incidence] 10 10
[kBq U235-
IR 1.55E-1 1.93E-3 4.17E-20.00E+00.00E+00.00E+00.00E+01.32E-2 3.15E-4 5.56E-10.00E+00.00E+01.42E-2-7.99E-2-1.89E-1
Eq.]
- -
ETP-fw [CTUe] 3.61E+15.29E+06.00E+00.00E+00.00E+00.00E+00.00E+02.27E-1 8.64E-19.56E+00.00E+00.00E+01.09E+1
3.31E+03.63E+0
1.09E- 5.94E- 6.27E- 1.79E- 2.64E- 5.80E- -4.09E-
HTP-c [CTUh] 1.61E-9 0.00E+00.00E+00.00E+00.00E+0 0.00E+00.00E+0 -1.01E-9
10 10 12 11 10 10 10
2.31E- 9.11E-
HTP-nc [CTUh] 1.34E-7 5.57E-9 2.41E-80.00E+00.00E+00.00E+00.00E+0 9.73E-90.00E+00.00E+05.94E-8-3.05E-8-6.65E-9
10 10
- -
SQP [-] 8.50E+22.48E+08.60E+10.00E+00.00E+00.00E+00.00E+01.69E-1 4.05E-17.12E+00.00E+00.00E+01.10E+0
1.73E+02.39E+0
PM = Potential incidence of disease due to PM emissions; IR = Potential Human exposure efficiency relative to U235; ETP-fw = Potential
Caption comparative Toxic Unit for ecosystems; HTP-c = Potential comparative Toxic Unit for humans (cancerogenic); HTP-nc = Potential
comparative Toxic Unit for humans (not cancerogenic); SQP = Potential soil quality index
Disclaimer 1 – for the indicator IRP : this impact category deals mainly with the eventual impact of low dose
ionizing radiation on human health of the nuclear fuel cycle. It does not consider effects due to possible nuclear
accidents, occupational exposure nor due to radioactive waste disposal in underground facilities. Potential
ionizing radiation from the soil, from radon and from some construction materials is also not measured by this
indicator.
Disclaimer 2 – for the indicators ADPE, ADPF, WDP, ETP-fw, HTP-c, HTP-nc, SQP : the results of this
environmental impact indicator shall be used with care as the uncertainties on these results are high or as there is
limited experienced with the indicator.
6. LCA: Interpretation
Looking at the overall life cycle for the scenario 1
(recycling), for most of the impact categories (except Within A1-A3, the pre-chains of the raw material have
for GWP-luluc, ADP-minerals&metals and WDP), the the most important impact in all impact categories
manufacturing of Duripanel B1 contributes to the except for GWP total/ ADP-fossil and EP-freshwater,
largest share (>50%) to the environmental followed by the energy consumption for the
performance. production. Transport to site (A2) has a negligible
influence (<2.5%) on the overall LCA results (except
The C3 phase has only minor impacts, except in the for GWP-luluc where it has little influence (<10%)).
category ODP and WDP relevant influences can be
seen, linked to the electricity use for shredding the The LCA for Duripanel B1 is in module A1 almost fully
waste material. determined by the pre-chains of the cement in all
impact categories except in the GWP-total and
Looking at the overall life cycle for the scenario 2 biogenic where the wood has high impact and in WDP
(landfill) in most of the impact categories (except for where the water consumed in the Duripanel process
GWP-total, biogenic and luluc, EP freshwater, ADP- has a very important contribution.
minerals&metals and WDP), the manufacturing of
Duripanel B1 contributes to the largest share (>50%)
to the environmental performance.
For the GWP-total and the GWP-biogenic, next to the
production phase, the main impacts occur in module
C4 linked to the EOL landfilling of the waste and re-
emission of organic carbon dioxide linked to it.
For the EP-freshwater, the production waste sent to
landfill in C4 is the main contributor.
The C4 phase has very important impacts (>25%) in
the categories GWP total and GWP biogenic and the
most important contribution (>50%) in EP freshwater.
9 Environmental Product Declaration Etex Germany Exteriors GmbH – Duripanel B1
7. Requisite evidence
Cu Cupper 0.016 mg/l
7.1 Testing pretreatment of substances used Mo Molybdenum <0.005 mg/l
Measurements according to the Waste Wood Ni Nickel 0.0465 mg/l
Ordinance are not relevant as no waste wood is used Hg Mercury <0.2 mg/l
in the manufacture of Duripanel B1 wood cement Se Selenium <0.002 mg/l
products. Zn Zinc <0.0176 mg/l
7.2 Leaching 7.3 VOC emissions
Measurement in accordance with EN 71-3, University Measurements in line with the AgBB diagram; Eurofins
of Osnabrück, Institute of Chemistry, Osnabrück; Product Testing A/S, Galten, Denmark 29.05.2008.
03.02.2000
Results : the analysis results of the leaching of the AgBB overview of results (28 days [µg/m³])
examined boards showed that the limit values laid Name Value Unit
down in EN 71 were complied with. TVOC (C6 - C16) 160 μg/m3
Sum SVOC (C16 - C22) 0 - 0.5 μg/m3
Measurement in accordance with EN 12457-4, UCL R (dimensionless) 0.07 -
Umwelt Control Labor GmbH, Lünen; 23.07.2019 : VOC without NIK 16 μg/m3
Carcinogenic Substances 0 - 0.1 μg/m3
Name Value Unit AgBB overview of results (3 days [µg/m³])
Sb Antimony <0.001 mg/l
Name Value Unit
As Arsenic <0.001 mg/l
TVOC (C6 - C16) 540 μg/m3
Ba Barium 0.667 mg/l
Sum SVOC (C16 - C22) 0 - 0.5 μg/m3
Pb Lead 0.0487 mg/l
VOC without NIK 23 μg/m3
Cd Cadmium <0.0003 mg/l
Carcinogenic Substances 0 - 0.1 μg/m3
Cr Chromium <0.0077 mg/l
8. References
Standards EN 15804
EN 15804:2012+A2:2019, Sustainability of
DIN EN 1995-1-1/NA construction works — Environmental Product
DIN EN 1995-1-1/NA:2013-08, National Annex – Declarations — Core rules for the product category of
Nationally determined parameters – Eurocode 5: construction products.
Design of timber structures – Part 1-1: General –
Common rules and rules for buildings. EN 1995-1-1
EN 1995-1-1:2004/A2:2014, Eurocode 5: Design of
DIN 4102-1 timber structures – Part 1-1: General – Common rules
DIN 4102-1:1998, Fire behaviour of building materials and rules for buildings.
and elements - Classification of building materials -
Requirements and testing. EN 634-1
EN 634-1:1995, Cement-bonded particleboards -
EN ISO 14025 Specifications - Part 1: General requirements.
DIN EN ISO 14025:2011-10, Environmental labels and
declarations — Type III environmental declarations — EN 634-2
Principles and procedures. EN 634-2:2007, Cement-bonded particleboards -
Specifications - Part 2: Requirements for OPC bonded
EN 12457-4 particleboards for use in dry, humid and external
EN 12457-4:2002, Characterisation of waste. conditions.
Leaching. Compliance test for leaching of granular
waste materials and sludges. One stage batch test at a EN 71-3
liquid to solid ratio of 10 l/kg for materials with particle EN 71-3:2019, Safety of toys - Part 3: Migration of
size below 10 mm (without or with size reduction). certain elements.
EN 13501-1 ISO 12571
EN 13501-1:2018, Fire classification of construction DIN EN ISO 1271:2000, Hygrothermal performance of
products and building elements - Part 1: Classification building materials and products — Determination of
using data from reaction to fire tests. hygroscopic sorption properties.
EN 13986 ISO 12572
DIN EN 13986:2015-06, Wood-based panels for use in DIN EN ISO 12572:2001, Hygrothermal performance
construction - Characteristics, evaluation of conformity of building materials and products - Determination of
and marking. water vapour transmission properties - Cup method
10 Environmental Product Declaration Etex Germany Exteriors GmbH – Duripanel B1
ISO 14025 (http://www.gabi-
DIN EN ISO 14025:2011-10, Environmental labels and software.com/international/support/gabi/gabi-database-
declarations — Type III environmental declarations — 2020-lci-documentation/)
Principles and procedures.
ISO 9001 IBU 2016
UNI EN ISO 9001:2015 September 2015, Quality Institut Bauen und Umwelt e.V.: General Programme
management systems - Requirements Instructions for the Preparation of EPDs at the Institut
Bauen und Umwelt e.V. Version 1.1, Berlin: Institut
ISO 14001 Bauen und Umwelt e.V., 2016.
UNI EN ISO 14001:2015, Environmental management (http://www.ibu-epd)
systems - Requirements with guidance for use.
Ordinance on Biocide Products
OHSAS 18001 Regulation (EU) No 528/2012 of the European
OHSAS 18001:2007, Occupational Health and Safety Parliament and of the Council of 22 May 2012
Management Certification. concerning the making available on the market and
use of biocidal products.
Further References PCR Part A
PCR Part A: Calculation rules for the Life Cycle
AgBB Assessment and Requirements on the Background
Ausschuss zur gesundheitlichen Bewertung von Report according to EN 15 804+A2:2019, Version 1.0,
Bauprodukten, AgBB (eng. German Committee for Institut Bauen und Umwelt e.V., 2020.
health-related evaluation of building products.
PCR Part B
BBSR PCR Part B: requirements on the EPD for wood
BBSR table "Service lives of components for life cycle cement - mineral-bonded wooden composites, version
assessment according to Bewertungssystem 1.7, Institut Bauen und Umwelt e.V., 2019.
Nachhaltiges Bauen (BNB)" Sustainable Building
Information Portal by the Federal Ministry of Transport, REACH Regulation
Building and Urban Affairs (Bundesinstitut für Bau- Regulation (EU) No 1907/2006 of the European
,Stadt-und Raumforschung, BBSR). Parliament and of the Council of 18 December 2006
(https://www.nachhaltigesbauen.de/baustoff- concerning the Registration, Evaluation, Authorisation
undgebaeudedaten/ and Restriction of Chemicals (REACH), establishing a
nutzungsdauern-von-bauteilen.html) European Chemicals Agency, amending Directive
1999/45/EC and repealing Council Regulation (EEC)
Candidate list No 793/93 and Commission
Candidate List of substances of very high concern for Regulation (EC) No 1488/94 as well as Council
Authorisation, published on ECHA website, latest Directive 76/769/EEC and Commission Directives
version 19.01.2021. (https://echa.europa.eu/candidate- 91/155/EEC, 93/67/EEC, 93/105/EC and 2000/21/EC.
list-table)
TA Luft
CPR Technische Anleitung zur Reinhaltung der Luft, version
Construction Products Regulation, Regulation (EU) No 16.12.2020.
305/2011 of the European Parliament and of the
Council of 9 March 2011 laying TRGS 900
down harmonized conditions for the marketing of TRGS 900: Edition: January 2006
construction products and repealing Council Directive BArBl. issue 1/2006 p. 41-55
89/106/ EEC Text with EEA relevance. corrected GMBl 2020 S. 276 [No. 12-13] of 30.03.2020
amended and supplemented: GMBl 2020, 815-816
Eurofins Product Testing A/S [No. 38] of 02.10.2020
Eurofins Product Testing A/S, Smedeskovvej 38, 8464 https://www.baua.de/DE/Angebote/Rechtstexte-und-
Galten, Denmark. Technische-Regeln/Regelwerk/TRGS/TRGS-900.html
Waste Wood Ordinance
GaBi ts software/ GaBi database Ordinance on requirements for the exploitation and
GaBi Software System and Database for Life Cycle disposal of waste wood of 15.08.2002.
Engineering, 1992-2020, Sphera Solutions GmbH,
Leinfelden-Echterdingen, with acknowledgement of Umwelt Control Labor GmbH
LBP University of Stuttgart, program version 9.5.2.49. Umwelt Control Labor GmbH, Postfach 2063, 44510
Database version 2020.1, SP40. Lünen, Deutschland.
GaBi documentation
GaBi dataset documentation for the software system
and databases, LBP, University of Stuttgart and
Sphera Solutions GmbH, Leinfelden-Echterdingen,
2020.
11 Environmental Product Declaration Etex Germany Exteriors GmbH – Duripanel B1
Publisher
Institut Bauen und Umwelt e.V. Tel +49 (0)30 3087748- 0
Panoramastr. 1 Fax +49 (0)30 3087748- 29
10178 Berlin Mail info@ibu-epd.com
Germany Web www.ibu-epd.com
Programme holder
Institut Bauen und Umwelt e.V. Tel +49 (0)30 - 3087748- 0
Panoramastr 1 Fax +49 (0)30 – 3087748 - 29
10178 Berlin Mail info@ibu-epd.com
Germany Web www.ibu-epd.com
Author of the Life Cycle
Assessment Tel +32 (0)15 71 82 83
Peggy Van De Velde Fax +32 (0)15 71 82 29
Bormstraat 24 Mail
2830 Tisselt peggy.vandevelde@etexgroup.c
Belgium om
Web www.etexgroup.com
Owner of the Declaration
Etex Building Performance Tel +32 2 778 12 11
International Fax +32 2 778 12 12
Marcel Demonque 500 r Mail info@etexgroup.com
84915 Avignon Cedex 9 Web http://www.etexgroup.com
France
