ENVIRONMENTAL PRODUCT DECLARATION
as per ISO 14025 and EN 15804+A2
Owner of the Declaration Adolf Würth GmbH & Co. KG
Publisher Institut Bauen und Umwelt e.V. (IBU)
Programme holder Institut Bauen und Umwelt e.V. (IBU)
Declaration number EPD-AWU-20230504-CBA4-EN
Issue date 14/09/2023
Valid to 13/09/2028
WIT-PE 1000
Adolf Würth GmbH & Co. KG
www.ibu-epd.com | https://epd-online.com
General Information
Adolf Würth GmbH & Co. KG WIT-PE 1000
Programme holder Owner of the declaration
IBU – Institut Bauen und Umwelt e.V. Adolf Würth GmbH & Co. KG
Hegelplatz 1 Reinhold-Würth-Str. 12-17
10117 Berlin 74653 Künzelsau
Germany Germany
Declaration number Declared product / declared unit
EPD-AWU-20230504-CBA4-EN The declared product is the two-component reaction resin mortar "WIT-PE
1000". The declared unit is based on 1 kg reaction resin product in the
ratio at which the two components must be mixed before use. The
packaging is also included in the calculation, since the product is sold by
Adolf Würth GmbH & Co. KG with its packaging. The declared unit is
indicated in [kg].
This declaration is based on the product category rules: Scope:
Reaction resin products, 01/08/2021 This document covers the two-component reaction resin mortar "WIT-PE
(PCR checked and approved by the SVR) 1000". To prepare the life cycle assessment [LCA], specific data were
collected from the manufacturing facility in Willich, Germany. The
assessment is based on data from 2020 which correspond to the yearly
Issue date average.
The owner of the declaration shall be liable for the underlying information
14/09/2023
and evidence; the IBU shall not be liable with respect to manufacturer
information, life cycle assessment data and evidences.
Valid to
The EPD was created according to the specifications of EN 15804+A2. In
13/09/2028 the following, the standard will be simplified as EN 15804.
Verification
The standard EN 15804 serves as the core PCR
Independent verification of the declaration and data according to ISO
14025:2011
internally X externally
Dipl.-Ing. Hans Peters
(Chairman of Institut Bauen und Umwelt e.V.)
Florian Pronold Angela Schindler,
(Managing Director Institut Bauen und Umwelt e.V.) (Independent verifier)
1 Environmental Product Declaration - Adolf Würth GmbH & Co. KG - WIT-PE 1000
Product
+ 10°C 1680 min.
Product description/Product definition + 15°C 1080 min.
The declared product WIT-PE 1000 is a two-component + 20°C 720 min.
reaction resin mortar based on epoxy resin that is delivered in a + 25°C 540 min.
two-component plastic cartridge. The high-performance product + 35°C 360 min.
is applied through a static mixer using a manual, battery- + 40°C 240 min.
operated or pneumatic gun. It was specially developed for use
in securing threaded rods, rebar or internally threaded sleeves For more information, please refer to the relevant technical data
in concrete. sheet.
Marketing of the product in the EU/EFTA (except for
Switzerland) is governed by Regulation Product performance values in accordance with the Declaration
(EU) No. 305/2011 (CPR). The product requires a Declaration of Performance with regard to its principal characteristics
of Performance subject to ETA-19/0542 andETA-19/0543 and according to ETA-19/0542 and ETA-19/0543.
CE marking.
Base materials/Ancillary materials
The declared product WIT-PE 1000 is delivered as a two-
Application component plastic cartridge and consists of a resin component
The WIT-PE 1000 injection system is used to safely secure and a curing agent component in a 3:1 volume ratio. The mixing
threaded rods, internally threaded sleeves and post-mortared ratio between the resin component and the curing agent
rebar connections in cracked and uncracked C20/25 to C50/60 component is set automatically as the
concrete for a useful life of up to 100 years, and is suitable for product is pushed out of the cartridge. Curing begins
installation in hammer-drilled (standard SDS and hollow bit) and immediately after the components are mixed.
diamond-drilled holes at environmental temperatures between
0°C and 40°C. The WIT-PE 1000 system has ETA assessments 1) "This product/article/at least one partial article contains
and ICC certifications, including seismic category C1 and C2 for substances in the ECHA candidate list of substances of very
anchoring from M8 to M30 and for rebar connections including high concern (SVHC) (17 January 2023) above a concentration
seismic conditions from 8mm to 40mm, and can be rated for fire of 0.1% by mass: no."
conditions.
2) "This product/article/at least one partial article contains other
Technical Data
CMR substances in categories 1A or 1B which are not on the
The following structural properties are relevant for the declared candidate list, exceeding 0.1 percentage by mass: no"
product WIT-PE 1000 as delivered:
Construction Data 3) "Biocide products were added to this construction product or
it has been treated with biocide products (this then concerns a
Name Value Unit
treated product as defined by the (EU) Regulation on Biocidal
Density acc. to DIN 51757 for mixing the two
1.4 g/cm³ Products No. 528/2012): no"
components
Compressive strength acc. to DIN EN 196 Part 1 121.8N/mm² The product considered in this EPD contains individual
Flexural strength acc. to DIN EN 196 Part 1 66 N/mm² components in the following ranges:
Storage:
Resin component:
Store in a cool, dry and dark place; storage temperature: +5°C
Epoxy resin: 40 to 75% by weight
to +35°C
Mineral fillers: 30 to 40% by weight
Other components: < 5% by weight
Shelf life:
24 months in cartridge systems
Curing agent component:
Various polyamines: 40 to 50% by weight
Gel and working time:
Mineral fillers: 30 to 50% by weight
0°C 90 min.
Other components: < 5% by weight
+ 5°C 80 min.
+ 10°C 60 min.
Reference service life
+ 15°C 40 min.
The declared product WIT-PE 1000 may be exposed to a wide
+ 20°C 30 min.
range of environmental conditions during the use phase. Its
+ 25°C 12 min.
expected reference service life depends on the specific
+ 35°C 8 min.
installation situation and on the product's resulting exposure.
+ 40 °C 8 min.
The main factors influencing service life
are weather conditions and mechanical and chemical stresses.
Curing time in dry substrate:
0°C 8640 min.
+ 5°C 2880 min.
LCA: Calculation rules
based on 1 kg reaction resin product in the ratio at which the
Declared Unit two components must be mixed before use. The mass mixing
The product declared is a two-component reaction resin mortar ratio between the resin component and the curing agent
with the product name WIT-PE 1000. The declared unit is component is 4:1 (volume ratio 3:1). The packaging is also
2 Environmental Product Declaration - Adolf Würth GmbH & Co. KG - WIT-PE 1000
included in the calculation at 0.1435 kg per 1 kg of reaction Figure 1 Information modules A1 to A3 of the product
resin product. The declared unit data are presented in the table
below:
Declared unit data
Name Value Unit
Declared unit 1 kg
System boundary
Type of EPD: Cradle to factory gate with options. The following
information modules are defined as system boundaries in this Figure 2 Information modules A1 to A3 of the packaging
study:
Information modules C1 to C4 document
Production stage (A1–A3): deconstruction/demolition for removal from the building,
• A1, Raw material extraction, transport to waste disposal, waste processing and product
• A2, Transport to the manufacturer, disposal. Reuse, recovery and recycling potential are
• A3, Manufacturing. documented in information module D.
Geographic Representativeness
End of life (C1-C4):
Land or region, in which the declared product system is
• C1, Deconstruction/demolition,
manufactured, used or handled at the end of the product´s
• C2, Transport,
lifespan: Germany
• C3, Waste processing,
• C4, Disposal.
Comparability
Reuse, recovery and recycling potential (D) Basically, a comparison or an evaluation of EPD data is only
possible if all the data sets to be compared were created
To precisely determine the indicators and environmental according to EN 15804 and the building context, respectively
impacts of the declared unit, a total of 8 information modules the product-specific characteristics of performance, are taken
are considered. The information modules A1 to A3 describe the into account.
material provision, the transport to the production site, as well The background datasets from the LCA for Experts and
as the production processes of the product itself. ecoinvent 3.9.1 databases, which this study also draws on, are
documented at the following site (Sphera). 2023.1
The precursor products are sourced from Germany. Transport http://www.gabi-software.com/deutsch/index/ (ecoinvent 3.9.1).
is exclusively done by truck. The following process diagrams http://ecoquery.ecoinvent.org/3.9.1/cutoff/search
illustrate the underlying production process.
LCA: Scenarios and additional technical information
End of Life (C1–C4)
Characteristic product properties of biogenic carbon
The product is demolished by using an electric chisel. The
No renewable raw materials are used in the product or the
electrical energy consumption for this tool is estimated at 0.05
packaging. The biogenic carbon value is therefore reported as
MJ for the declared unit. The power consumption is calculated
zero.
using a European energy mix. Construcion waste is transported
200 km by truck to a waste treatment facility. At the waste
treatment facility, the construction waste is shredded and then
Packaging per declared unit disposed in a landfill.
Name Value Unit Name Value Unit
Packaging PP 0.1188 kg Collected as mixed construction waste 1 kg
Packaging PA6 0.0082 kg Shredding 1 kg
Packaging PE-LD 0.0165 kg Disposal in landfill 1 kg
3 Environmental Product Declaration - Adolf Würth GmbH & Co. KG - WIT-PE 1000
zero.
Reuse, recovery and recycling potential (D), relevant
scenario specifications Name Value Unit
The product has no reuse, recovery or recycling potential. Reuse, recovery and recycling potential 0 kg
Information module D is therefore declared and reported as
4 Environmental Product Declaration - Adolf Würth GmbH & Co. KG - WIT-PE 1000
LCA: Results
The results in this calculation refer to the characterisation factors EN 15840+A2/EF 3.1.
DESCRIPTION OF THE SYSTEM BOUNDARY (X = INCLUDED IN LCA; MND = MODULE OR INDICATOR NOT DECLARED; MNR
= MODULE NOT RELEVANT)
Benefits and
Construction loads beyond
Product stage Use stage End of life stage
process stage the system
boundaries
la ire ta m w a Ry lp p u s tro p s n a rT g n iru tc a fu n a M e h t m o rf tro p s n a rTe tis e h t o t e ta g y lb m e s s A e s U e c n a n e tn ia M ria p e R tn e m e c a lp e R tn e m h s ib ru fe R y g re n e la n o ita re p Oe s u re ta w la n o ita re p Oe s u n o itc u rts n o c -e Dn o itilo m e d tro p s n a rT g n is s e c o rp e ts a W la s o p s iD -e s u e R-y re v o c e R-g n ilc y c e Rla itn e to p
A1 A2 A3 A4 A5 B1 B2 B3 B4 B5 B6 B7 C1 C2 C3 C4 D
X X X MND MND MND MND MNR MNR MNR MND MND X X X X X
RESULTS OF THE LCA - ENVIRONMENTAL IMPACT according to EN 15804+A2: 1 kg WIT-PE 1000
Parameter Unit A1-A3 C1 C2 C3 C4 D
Global Warming Potential total (GWP-total) kg CO 2 eq 4.1E+00 4.58E-03 1.75E-02 2.58E-03 1.46E-02 0
Global Warming Potential fossil fuels (GWP-fossil) kg CO 2 eq 3.97E+00 4.53E-03 1.73E-02 2.56E-03 1.46E-02 0
Global Warming Potential biogenic (GWP-biogenic) kg CO 2 eq 1.26E-01 4.91E-05 0 0 0 0
Global Warming Potential luluc (GWP-luluc) kg CO 2 eq 8.91E-04 4.87E-07 1.58E-04 1.92E-05 4.53E-05 0
Depletion potential of the stratospheric ozone layer (ODP) kg CFC11 eq 2.19E-10 8.27E-14 1.49E-15 4.28E-15 3.71E-14 0
Acidification potential of land and water (AP) mol H+ eq 5.13E-03 9.57E-06 6.48E-05 1.34E-05 1.03E-04 0
Eutrophication potential aquatic freshwater (EP-freshwater) kg P eq 2.24E-05 1.67E-08 6.21E-08 8.71E-09 2.93E-08 0
Eutrophication potential aquatic marine (EP-marine) kg N eq 1.76E-03 2.29E-06 3.03E-05 6.13E-06 2.67E-05 0
Eutrophication potential terrestrial (EP-terrestrial) mol N eq 1.89E-02 2.39E-05 3.39E-04 6.77E-05 2.94E-04 0
Formation potential of tropospheric ozone photochemical oxidants kg NMVOC
5.94E-03 6.11E-06 5.84E-05 1.66E-05 8.06E-05 0
(POCP) eq
Abiotic depletion potential for non fossil resources (ADPE) kg Sb eq 2.08E-07 6.95E-10 1.1E-09 2.74E-09 6.72E-10 0
Abiotic depletion potential for fossil resources (ADPF) MJ 8.8E+01 9.43E-02 2.32E-01 5.04E-02 1.94E-01 0
m3 world eq
Water use (WDP) 1.21E-01 9.98E-04 1.96E-04 4.98E-04 1.6E-03 0
deprived
RESULTS OF THE LCA - INDICATORS TO DESCRIBE RESOURCE USE according to EN 15804+A2: 1 kg WIT-PE 1000
Parameter Unit A1-A3 C1 C2 C3 C4 D
Renewable primary energy as energy carrier (PERE) MJ 8.76E+00 5.64E-02 1.64E-02 4.68E-03 3.16E-02 0
Renewable primary energy resources as material utilization
MJ 0 0 0 0 0 0
(PERM)
Total use of renewable primary energy resources (PERT) MJ 8.76E+00 5.64E-02 1.64E-02 4.68E-03 3.16E-02 0
Non renewable primary energy as energy carrier (PENRE) MJ 6.69E+01 9.43E-02 2.32E-01 5.05E-02 1.94E-01 0
Non renewable primary energy as material utilization (PENRM) MJ 2.11E+01 0 0 0 0 0
Total use of non renewable primary energy resources (PENRT) MJ 8.81E+01 9.43E-02 2.32E-01 5.05E-02 1.94E-01 0
Use of secondary material (SM) kg 0 0 0 0 0 0
Use of renewable secondary fuels (RSF) MJ 0 0 0 0 0 0
Use of non renewable secondary fuels (NRSF) MJ 0 0 0 0 0 0
Use of net fresh water (FW) m3 1.18E-02 4.55E-05 1.81E-05 1.44E-05 4.9E-05 0
RESULTS OF THE LCA – WASTE CATEGORIES AND OUTPUT FLOWS according to EN 15804+A2:
1 kg WIT-PE 1000
Parameter Unit A1-A3 C1 C2 C3 C4 D
Hazardous waste disposed (HWD) kg 7.4E-09 7.38E-12 8.59E-13 1.31E-13 4.23E-12 0
Non hazardous waste disposed (NHWD) kg 6.94E-02 6.91E-05 3.35E-05 1.33E-05 9.71E-01 0
Radioactive waste disposed (RWD) kg 1.31E-03 1.5E-05 3E-07 6.77E-07 2.21E-06 0
Components for re-use (CRU) kg 0 0 0 0 0 0
Materials for recycling (MFR) kg 0 0 0 0 0 0
Materials for energy recovery (MER) kg 0 0 0 0 0 0
Exported electrical energy (EEE) MJ 0 0 0 0 0 0
Exported thermal energy (EET) MJ 0 0 0 0 0 0
RESULTS OF THE LCA – additional impact categories according to EN 15804+A2-optional:
1 kg WIT-PE 1000
Parameter Unit A1-A3 C1 C2 C3 C4 D
Disease
Incidence of disease due to PM emissions (PM) ND ND ND ND ND ND
incidence
Human exposure efficiency relative to U235 (IR) kBq U235 eq ND ND ND ND ND ND
Comparative toxic unit for ecosystems (ETP-fw) CTUe ND ND ND ND ND ND
Comparative toxic unit for humans (carcinogenic) (HTP-c) CTUh ND ND ND ND ND ND
5 Environmental Product Declaration - Adolf Würth GmbH & Co. KG - WIT-PE 1000
Comparative toxic unit for humans (noncarcinogenic) (HTP-nc) CTUh ND ND ND ND ND ND
Soil quality index (SQP) SQP ND ND ND ND ND ND
Disclaimer 2 - applies to the following indicators: 'Abiotic shortage potential - non-fossil resources', 'Abiotic shortage potential - fossil
fuels', 'Water deprivation potential (users)', 'Potential comparative toxic unit for ecosystems', 'Potential comparative toxic unit for human
health - carcinogenic effects', 'Potential comparative toxic unit for human health - non-carcinogenic effects', 'Potential soil quality index'.
The results of this environmental impact indicator shall be used with care, as the uncertainties of the results are high and as there is
limited experience with the indicator.
References
DIN 51757 Background database: ecoinvent 3.9.1 Ziirich: ecoinvent (Ed.)
DIN 51757:2011-01 http://www.ecoinvent.org
Testing of mineral oils and related materials - Determination of (26 May 2023)
density.
ETA-19/0542
EN 196 European Technical Assessment
DIN EN 196-1:2016-11
Methods of testing cement - Part 1: Determination of strength. ETA-19/0543
European Technical Assessment
EN 15804 IBU 2021
EN 15804+A2:2019+AC:2021, Sustainability of construction Institut Bauen und Umwelt e.V.: General guidance for the EPD
works - Environmental product declarations - Core rules for the programme of the Institut Bauen und Umwelt e.V., Version 2.0,
product category of construction products. Berlin: Institut Bauen und Umwelt e.V., 2021. www.ibu-epd.com
EN/TR 15941
CEN/TR 15941:2010-03: Sustainability of construction works - PCR Part A
Environmental product declarations - Methodology for selection Product Category Rules for Building-Related Products and
and use of generic data Services - Calculation Rules for Life Cycle Assessment and
Requierements on the Project Report V1.3, Institut Bauen und
ISO 14025 Umwelt e.V., 08.2022
DIN EN ISO 14025:2011-10, Environmental labels and
declarations - Type III PCR: Reaction resin products
environmental declarations - Principles and procedures. Guidance-Texts for Building-Related Products and Services-
PART B: Requirements on the Environmental Product
ISO 14044 Declarations for Reaction Resin Products,1 August 2021
DIN EN ISO 14044:2006-10, Environmental management - Life
cycle assessment - Requirements and guidelines. Sphera
LCA for Experts: 2023.1
Further references Leinfelden-Echterdingen; Sphera
Solution GmbH (Ed.)
ECHA candidates list http://www. gabi-software.com/deutsch/index/
https://echa.europa.eu/de/candiate-list-substances-in-articles (26 May 2023)
ECHA list Regulation (EU) No. 305/2011 (CPR)
https://echa.europa.eu/de/candiate-list-table
Regulation (EU) No. 528/2012 (Biocidal Products Regulation)
ecoinvent 3.9.1
6 Environmental Product Declaration - Adolf Würth GmbH & Co. KG - WIT-PE 1000
Publisher
Institut Bauen und Umwelt e.V. +49 (0)30 3087748- 0
Hegelplatz 1 info@ibu-epd.com
10117 Berlin www.ibu-epd.com
Germany
Programme holder
Institut Bauen und Umwelt e.V. +49 (0)30 3087748- 0
Hegelplatz 1 info@ibu-epd.com
10117 Berlin www.ibu-epd.com
Germany
Author of the Life Cycle Assessment
FIT-Umwelttechnik GmbH 05362 72 69 474
Westerstr. 13 bertram@fit-umwelttechnik.de
38442 Wolfsburg www.fit-umwelttechnik.com
Germany
Owner of the Declaration
Adolf Würth GmbH & Co. KG +49 7940/15-0
Reinhold-Würth-Str. 12-17 info@wuerth.com
74653 Künzelsau www.wuerth.de
Germany
7 Environmental Product Declaration - Adolf Würth GmbH & Co. KG - WIT-PE 1000
