ENVIRONMENTAL PRODUCT DECLARATION
as per ISO 14025 and EN 15804+A2
Owner of the Declaration Fletco Carpets A/S
Publisher Institut Bauen und Umwelt e.V. (IBU)
Programme holder Institut Bauen und Umwelt e.V. (IBU)
Declaration number EPD-FLE-20230274-CBC1-EN
Issue date 25.07.2023
Valid to 24.07.2028
Woven broadloom carpet, pile material solution-dyed polyamide
6.0 with a woven textile or a "Silent Bac" backing, both backings
with recycled content, maximum total pile weight 400 g/m²
Fletco Carpets A/S
www.ibu-epd.com | https://epd-online.com
General Information
Fletco Carpets A/S Woven broadloom carpet, pile material solution-
dyed polyamide 6.0 with a woven textile or a
"Silent Bac" backing, both backings with recycled
content, maximum total pile weight 400 g/m²
Programme holder Owner of the declaration
IBU – Institut Bauen und Umwelt e.V. Fletco Carpets A/S
Hegelplatz 1 Mads Clausens Vej 2
10117 Berlin 7441 Bording
Germany Denmark
Declaration number Declared product / declared unit
EPD-FLE-20230274-CBC1-EN 1 m2 woven broadloom carpet having a pile material of polyamide 6 and a
woven textile or a "Silent Bac" backing.
This declaration is based on the product category rules: Scope:
Floor coverings, 01.08.2021 The manufacturer declaration applies to the specific woven broadloom
(PCR checked and approved by the SVR) carpet with a woven textile or a "Silent Bac" backing and a total pile weight
of 400 g/m2 .
The carpet is woven in the Fletco manufacturing site Bording, Denmark
Issue date and it is precoated and back-coated in the Foamtex site, Bording,
Denmark.
25.07.2023
The declaration is only valid in conjunction with a valid GUT-PRODIS
license of the product.
The owner of the declaration shall be liable for the underlying information
Valid to
and evidence; the IBU shall not be liable with respect to manufacturer
24.07.2028 information, life cycle assessment data and evidences.
The EPD was created according to the specifications of EN 15804+A2. In
the following, the standard will be simplified as EN 15804.
Verification
The standard EN 15804 serves as the core PCR
Independent verification of the declaration and data according to ISO
14025:2011
internally X externally
Dipl.-Ing. Hans Peters
(Chairman of Institut Bauen und Umwelt e.V.)
Florian Pronold Angela Schindler,
(Managing Director Institut Bauen und Umwelt e.V.) (Independent verifier)
Environmental Product Declaration - Fletco Carpets A/S - Woven broadloom carpet, pile material solution-dyed polyamide 6.0 with a woven textile or a "Silent Bac"
1 backing, both backings with recycled content, maximum total pile weight 400 g/m²
Product
Performance data of the product in accordance with the
Product description/Product definition declaration of performance with respect to its essential
Woven broadloom carpet having a pile material of solution-dyed characteristics according to EN 14041: 2018-05, Resilient,
polyamide 6 and a woven textile or a "Silent Bac" backing with textile and laminate floor coverings - Essential characteristics.
recycled content. The maximum total pile weight is 400 g/m2. Additional product properties in accordance with EN 1307 can
For the placing on the market of the specific product in the be found on the Product Information System PRODIS using the
European Union/European Free Trade Association (EU/EFTA) PRODIS registration number of the product (www.pro-dis.info)
(with the exception of Switzerland) Regulation (EU) No. or on the manufacturer's technical information section.
305/2011 Construction Product Regulation (CPR) applies. The
product needs a Declaration of Performance (DoP) taking into Base materials/Ancillary materials
consideration EN 14041:2018-05, Resilient, textile and laminate Values for the carpet with Silent Bac backing.
floor coverings - Essential characteristics, and the CE-marking. Name Value Unit
The DoP of the product can be found on the manufacturer's
Polyamide 6 19.3 %
technical information section. For the application and use of the
Polyester 35.3 %
product the respective national provisions apply.
Polymer dispersion (solid content) 15.4 %
Application Mineral filler 21.7 %
According to the use class as defined in EN 1307 the products Aluminium hydroxide 6.9 %
can be used in all professional areas with heavy use which
Additives 1.4 %
require class 33 or less.
The specific product covered by the EPD contains substances
listed in the ECHA candidate list (26.07.2022) or other
carcinogenic, mutagenic or reprotoxic (CMR) substances in
categories 1A or 1B which are not on the candidate list
exceeding 0.1 percentage by mass: no
Technical Data
The products are registered in the GUT-PRODIS Information
System. The PRODIS system ensures compliance with
Constructional data according to EN 1307 limitations of various chemicals and Volatile Organic Compound
(VOC)-emissions and a ban on the use of all substances that
Name Value Unit
are listed as 'Substances of Very High Concern' (SVHC) under
Product Form Broadloom carpet on rolls of 4 m width -
REACH.
Type of
Woven carpet -
manufacture Reference service life
Dyeing method solution-dyed yarn - The service life of textile floor coverings strongly depends on
the correct installation taking into account the declared use
Yarn type Polyamide 6 -
classification and the adherence to cleaning and maintenance
woven textile backing or felt backing
Secondary instructions.
made of recycled -
backing A calculation of the reference service life according to ISO
polyethylenterephthalate (PET)
15686 is not possible. Alternatively, a reference service life of
Total pile
400 g/m² 10 years can be assumed, during which the functional and
weight max.
visual quality is guaranteed (BNB, Nutzungsdauer von
Total carpet Bauteilen). The technical service life can be significantly longer.
2100 g/m2
weight max.
LCA: Calculation rules
Declared Unit System boundary
Type of EPD:
Values for the carpet with Silent Bac backing. Cradle-to-gate with options, modules C1-C4, module D, and
Name Value Unit additional modules A4, A5, B1, B2.
Declared unit 1 m2
System boundaries of modules A, B, C, D:
Grammage 2.1 kg/m2 Modules C3, C4 and D are indicated separately for three end-
Layer thickness 0.004 m of-life scenarios:
Gross density 540 kg/m3
1 - landfill disposal
The declared unit refers to 1 m2 produced textile floor covering. 2 - municipal waste incineration
The Output of module A5 'Assembly' is 1 m2 installed textile 3 - recovery in a cement plant
floor covering.
The layer thickness of the specific product covered by the EPD A1-A3 Production:
can be found on the Product Information System PRODIS using Energy supply and production of the basic material, processing
the PRODIS registration number of the product (www.pro- of secondary material, auxiliary material, transport of the
dis.info) or on the manufacturer's technical information section. material to the manufacturing site, emissions, waste water
treatment, packaging material and waste processing up to the
landfill disposal of residual waste (except radioactive waste).
Benefits for generated electricity and steam due to the
Environmental Product Declaration - Fletco Carpets A/S - Woven broadloom carpet, pile material solution-dyed polyamide 6.0 with a woven textile or a "Silent Bac"
2 backing, both backings with recycled content, maximum total pile weight 400 g/m²
incineration of production waste are aggregated. Transport of the carpet waste to a landfill, to the municipal
waste incineration plant (MWI) or to the waste collection facility
A4 Transport: for recycling.
Transport of the packed textile floor covering from factory gate
to the place of installation. C3 Waste processing:
C3-1: Landfill disposal needs no waste processing.
A5 Installation: C3-2: Impact from waste incineration (plant with R1>0.6),
Installation of the textile floor covering, processing of generated electricity and steam are listed in the result table as
installation waste and packaging waste up to the landfill exported energy.
disposal of residual waste (except radioactive waste), the C3-3: Collection of the carpet waste for recovery in the cement
production of the amount of carpet that occurs as installation industry, waste processing (granulating), transport to the
waste including its transport to the place of installation. cement plant, emissions from the incineration.
Generated electricity and steam due to the incineration of
waste are listed in the result table as exported energy. C4 Disposal:
Preparation of the floor and auxiliary materials (adhesives, C4-1: Impact from landfill disposal,
fixing agents, PET connectors) are beyond the system C4-2: The carpet waste leaves the system in module C3-2,
boundaries and not taken into account. C4-3: The pre-processed carpet waste leaves the system in
module C3-3.
B1 Use:
Indoor emissions during the use stage. After the first year, no D Recycling potential:
product-related Volatile Organic Compound (VOC) emissions Calculated benefits result from materials exclusive secondary
are relevant due to known VOC decay curves of the product. materials (net materials).
D-A5: Benefits for generated energy due to incineration of
B2 Maintenance: packaging and installation waste (incineration plant with R1 >
Cleaning of the textile floor covering for a period of 1 year: 0.6),
Vacuum cleaning – electricity supply D-1: Benefits for generated energy due to landfill disposal of
Wet cleaning – electricity, water consumption, production of the carpet waste at the end of life,
cleaning agent, waste water treatment. D-2: Benefits for generated energy due to incineration of carpet
The declared values in this module have to be multiplied by the waste at the end-of-life (incineration plant with R1 > 0.6),
assumed service life of the floor covering in the building in D-3: Benefits for saved fossil energy and saved inorganic
question. material due to recovery of the carpet in a cement plant.
B3 - B5: Geographic Representativeness
The modules are not relevant within the assumed reference Land or region, in which the declared product system is
service life of 10 years. manufactured, used or handled at the end of the product´s
lifespan: Europe
B6 - B7:
No energy and water input are required for the operation of the
Comparability
carpet in the use stage. The modules are not relevant and not
Basically, a comparison or an evaluation of EPD data is only
declared.
possible if all the data sets to be compared were created
according to EN 15804 and the building context, respectively
C1 De-construction:
the product-specific characteristics of performance, are taken
The floor covering is de-constructed manually and no additional
into account. Background data are taken from the GaBi
environmental impact is caused.
database 2022-2.
C2 Transport:
LCA: Scenarios and additional technical information
agents, PET connectors etc.) are not taken into account.
Characteristic product properties of biogenic carbon
Biogenic carbon is neither contained in the product nor in the
Maintenance (B2)
packaging material.
The values for cleaning refer to 1 m2 floor covering per year.
Depending on the application based on ISO 10874, the
technical service life recommended by the manufacturer and
Transport to the construction site (A4)
the anticipated strain on the floor by customers, the case-
Name Value Unit specific useful life can be established. Based on this useful life
Litres of fuel (truck, EURO 0-6 mix) 0.0051 l/100km the effects of module B2 need to be calculated in order to
obtain the overall environmental impacts.
Transport distance 700 km
Capacity utilisation (including empty runs) 55 % Name Value Unit
Maintenance cycle (vacuum cleaning) 208 Number /year
Installation in the building (A5)
Maintenance cycle (wet cleaning) 1,5 Number /year
Name Value Unit Water consumption (wet cleaning) 0.004 m3
Material loss 0.193 kg
Cleaning agent (wet cleaning) 0.09 kg
Polyethylene packaging waste and installation waste are Electricity consumption 0.314 kWh
considered to be incinerated in a municipal waste incineration
For further information on cleaning and maintenance see
plant.
www.fletcocarpets.com
Preparation of the floor and auxiliaries (adhesives, fixing
Environmental Product Declaration - Fletco Carpets A/S - Woven broadloom carpet, pile material solution-dyed polyamide 6.0 with a woven textile or a "Silent Bac"
3 backing, both backings with recycled content, maximum total pile weight 400 g/m²
If combinations of these scenarios have to be calculated this
should be done according to the following scheme:
Service life
EOL-impact = x % impact (Scenario 1)
Name Value Unit
+ y % impact (Scenario 2)
Life Span (according to BBSR) 10 a + z % impact (Scenario 3)
Corresponds to the with x % + y % + z % = 100 %
Declared product properties (at
the gate) and finishes specifications of EN - Name ValueUnit
1307
Collected as mixed construction waste (scenarios 1
An assumed quality of work, Conforms to the and 2) 2.1 kg
when installed in accordance
manufacturer's - Collected separately (scenario 3) 2.1 kg
with the manufacturer’s
instructions Landfilling (scenario 1) 2.1 kg
instructions
Energy recovery (scenario 2) 2.1 kg
Usage conditions, e.g. Use in areas defined by
frequency of use, mechanical the use class according - Energy recovery (scenario 3) 1.5 kg
exposure to EN 1307 Recycling (scenario 3) 0.6 kg
Maintenance e.g. required According to the
frequency, type and quality and manufacturers - Reuse, recovery and/or recycling potentials (D), relevant
replacement of components instructions scenario information
Recovery or recycling potentials due to the three end-of-life
End of Life (C1-C4)
scenarios (module C) are indicated separately.
Three different end-of-life scenarios are declared and the
results are indicated separately in module C.
Recycling in the cement industry (scenario 3)
Each scenario is calculated as a 100 % scenario.
The organic material of the carpet is used as an alternative fuel
Scenario 1: 100 % landfill disposal
in a cement kiln. It mainly substitutes for lignite (68.8 %), hard
Scenario 2: 100 % municipal waste incineration (MWI)
coal (23.6 %) and petrol coke (7.6 %). The inorganic material is
with R1>0.6
substantially integrated into the cement clinker and substitutes
Scenario 3: 100 % recovery in the cement industry
for original material input. VDZ e.V.
Environmental Product Declaration - Fletco Carpets A/S - Woven broadloom carpet, pile material solution-dyed polyamide 6.0 with a woven textile or a "Silent Bac"
4 backing, both backings with recycled content, maximum total pile weight 400 g/m²
LCA: Results
The declared result figures in module B2 have to be multiplied by the assumed service life (in years) of the floor covering in the building
under consideration.
Information on non-relevant modules:
Modules B3 - B7 are not relevant during the service life of the carpet.
Modules C3/1, C4/2 and C4/3 cause no additional impact (see chapter "LCA: Calculation rules" in this document).
Module C2 represents the transport for scenarios 1, 2 and 3. The values in column D result from module A5.
DESCRIPTION OF THE SYSTEM BOUNDARY (X = INCLUDED IN LCA; ND = MODULE OR INDICATOR NOT DECLARED; MNR =
MODULE NOT RELEVANT)
Benefits and
Construction loads beyond
Product stage Use stage End-of-life stage
process stage the system
boundaries
la ire ta m w a Ry lp p u s tro p s n a rT g n iru tc a fu n a M e h t m o rf tro p s n a rTe tis e h t o t e ta g y lb m e s s A e s U e c n a n e tn ia M ria p e R tn e m e c a lp e R tn e m h s ib ru fe R y g re n e la n o ita re p Oe s u re ta w la n o ita re p Oe s u n o itc u rts n o c -e Dn o itilo m e d tro p s n a rT g n is s e c o rp e ts a W la s o p s iD -e s u e R-y re v o c e R-g n ilc y c e Rla itn e to p
A1 A2 A3 A4 A5 B1 B2 B3 B4 B5 B6 B7 C1 C2 C3 C4 D
X X X X X X X MNR MNR MNR MND MND X X X X X
RESULTS OF THE LCA - ENVIRONMENTAL IMPACT according to EN 15804+A2: 1 m² floor covering
Parameter Unit A1-A3 A4 A5 B1 B2 C1 C2 C3/2 C3/3 C4/1 D D/1 D/2 D/3
GWP-total kg CO 2 eq 8.13E+00 1.3E-01 1.17E+00 0 5.49E-01 0 7.28E-03 3.39E+003.42E+00 1.5E-01 -1.19E-01 0 -7E-01 -2.07E-01
GWP-fossil kg CO 2 eq 8.05E+00 1.27E-01 1.16E+00 0 3.48E-01 0 7.14E-03 3.39E+003.42E+00 1.5E-01 -1.18E-01 0 -6.96E-01 -2.07E-01
GWP-
biogenic kg CO 2 eq 7.79E-02 1.65E-03 7.2E-03 0 4.16E-03 0 9.25E-05 3.15E-04 6.45E-04 -2.47E-08 -6.03E-04 0 -3.53E-03 -2.49E-04
GWP-luluc kg CO 2 eq 3.45E-03 7.2E-04 3.85E-04 0 1.96E-01 0 4.05E-05 6.95E-05 1.73E-04 7.4E-05 -1.3E-05 0 -7.58E-05 -9.99E-05
kg CFC11
ODP 4.4E-09 7.74E-15 3.96E-10 0 3.42E-08 0 4.35E-16 2.73E-13 4.35E-13 2.04E-13 -7.96E-13 0 -4.65E-12 -3.12E-13
eq
AP mol H+ eq 1.37E-02 7.69E-04 1.51E-03 0 8.32E-04 0 4.32E-05 2.19E-03 2.33E-03 4.5E-04 -1.55E-04 0 -9.09E-04 -7.4E-04
EP-
kg P eq 4.13E-05 3.86E-07 3.78E-06 0 5.19E-06 0 2.17E-08 2.79E-07 3.65E-07 2.84E-05 -1.62E-07 0 -9.46E-07 -2.33E-07
freshwater
EP-marine kg N eq 4.18E-03 3.78E-04 5.09E-04 0 1.97E-04 0 2.12E-05 1.05E-03 1.11E-03 9.96E-05 -4.21E-05 0 -2.47E-04 -2.3E-04
EP-terrestrial mol N eq 4.07E-02 4.18E-03 5.18E-03 0 2.83E-03 0 2.35E-04 1.19E-02 1.25E-02 1.09E-03 -4.51E-04 0 -2.65E-03 -2.53E-03
kg
POCP NMVOC 1.32E-02 7.14E-04 1.51E-03 4.18E-04 9.83E-04 0 4.01E-05 2.69E-03 2.81E-03 3.21E-04 -1.18E-04 0 -6.93E-04 -6.93E-04
eq
ADPE kg Sb eq 1.36E-06 1.08E-08 1.25E-07 0 2.3E-07 0 6.07E-10 1.12E-08 1.57E-08 1.05E-08 -1.78E-08 0 -1.04E-07 -1.99E-08
-2.01E -1.18E -2.64E
ADPF MJ 1.59E+021.73E+001.46E+01 0 5.9E+00 0 9.7E-02 1.33E+001.77E+00 2.16E+00 0
+00 +01 +01
m3 world
WDP eq 1.04E+00 1.16E-03 1.39E-01 0 9.99E-02 0 6.49E-05 3.82E-01 3.84E-01 -1.61E-03 -1.24E-02 0 -7.24E-02 -3.08E-02
deprived
GWP = Global warming potential; ODP = Depletion potential of the stratospheric ozone layer; AP = Acidification potential of land and water; EP =
Eutrophication potential; POCP = Formation potential of tropospheric ozone photochemical oxidants; ADPE = Abiotic depletion potential for non-fossil
resources; ADPF = Abiotic depletion potential for fossil resources; WDP = Water (user) deprivation potential)
RESULTS OF THE LCA - INDICATORS TO DESCRIBE RESOURCE USE according to EN 15804+A2: 1 m² floor covering
Parameter Unit A1-A3 A4 A5 B1 B2 C1 C2 C3/2 C3/3 C4/1 D D/1 D/2 D/3
PERE MJ 2.69E+01 9.82E-02 2.46E+00 0 3.69E+00 0 5.51E-03 2.37E-01 3.61E-01 1.77E-01 -5.5E-01 0 -3.21E+00 -2.85E-01
PERM MJ 0 0 0 0 0 0 0 0 0 0 0 0 0 0
PERT MJ 2.69E+01 9.82E-02 2.46E+00 0 3.69E+00 0 5.51E-03 2.37E-01 3.61E-01 1.77E-01 -5.5E-01 0 -3.21E+00 -2.85E-01
PENRE MJ 1.28E+02 1.73E+00 1.62E+01 0 5.9E+00 0 9.72E-02 3.06E+01 3.1E+01 2.16E+00-2.01E+00 0 -1.18E+01-2.64E+01
-1.58E -2.92E -2.92E
PENRM MJ 3.08E+01 0 0 0 0 0 0 0 0 0 0
+00 +01 +01
PENRT MJ 1.59E+02 1.73E+00 1.46E+01 0 5.9E+00 0 9.72E-02 1.33E+00 1.78E+00 2.16E+00-2.01E+00 0 -1.18E+01-2.64E+01
SM kg 5.2E-01 0 4.68E-02 0 0 0 0 0 0 0 0 0 0 3.4E-01
RSF MJ 0 0 0 0 0 0 0 0 0 0 0 0 0 0
NRSF MJ 0 0 0 0 0 0 0 0 0 0 0 0 0 0
FW m3 4.18E-02 1.11E-04 4.84E-03 0 3.34E-03 0 6.23E-06 9.01E-03 9.13E-03 2.53E-05 -5.26E-04 0 -3.07E-03 -2.42E-03
PERE = Use of renewable primary energy excluding renewable primary energy resources used as raw materials; PERM = Use of renewable primary
energy resources used as raw materials; PERT = Total use of renewable primary energy resources; PENRE = Use of non-renewable primary energy
excluding non-renewable primary energy resources used as raw materials; PENRM = Use of non-renewable primary energy resources used as raw
materials; PENRT = Total use of non-renewable primary energy resources; SM = Use of secondary material; RSF = Use of renewable secondary fuels;
NRSF = Use of non-renewable secondary fuels; FW = Use of net fresh water
Environmental Product Declaration - Fletco Carpets A/S - Woven broadloom carpet, pile material solution-dyed polyamide 6.0 with a woven textile or a "Silent Bac"
5 backing, both backings with recycled content, maximum total pile weight 400 g/m²
RESULTS OF THE LCA – WASTE CATEGORIES AND OUTPUT FLOWS according to EN 15804+A2:
1 m² floor covering
Parameter Unit A1-A3 A4 A5 B1 B2 C1 C2 C3/2 C3/3 C4/1 D D/1 D/2 D/3
HWD kg 4.24E-04 8.29E-12 3.82E-05 0 4.19E-05 0 4.65E-13 1.86E-10 2.04E-10 3.33E-10 -2.72E-10 0 -1.61E-09 -1.37E-10
NHWD kg 1.62E-01 2.48E-04 4.67E-02 0 7.3E-03 0 1.39E-05 3.51E-01 3.51E-01 2.14E+00 -1.01E-03 0 -5.94E-03 -7.05E-02
RWD kg 4.14E-03 2.13E-06 3.78E-04 0 3.76E-04 0 1.2E-07 5.32E-05 8.53E-05 2.65E-05 -1.58E-04 0 -9.21E-04 -6E-05
CRU kg 0 0 0 0 0 0 0 0 0 0 0 0 0 0
MFR kg 0 0 0 0 0 0 0 0 3.4E-01 0 0 0 0 0
MER kg 0 0 0 0 0 0 0 0 0 0 0 0 0 0
EEE MJ 0 0 6.77E-01 0 0 0 0 4.73E+00 0 0 0 0 0 0
EET MJ 0 0 1.22E+00 0 0 0 0 8.64E+00 4.06E+01 0 0 0 0 0
HWD = Hazardous waste disposed; NHWD = Non-hazardous waste disposed; RWD = Radioactive waste disposed; CRU = Components for re-use;
MFR = Materials for recycling; MER = Materials for energy recovery; EEE = Exported electrical energy; EET = Exported thermal energy
RESULTS OF THE LCA – additional impact categories according to EN 15804+A2-optional:
1 m² floor covering
Parameter Unit A1-A3 A4 A5 B1 B2 C1 C2 C3/2 C3/3 C4/1 D D/1 D/2 D/3
Disease
PM 9.59E-08 4.45E-09 9.95E-09 0 6.84E-08 0 2.5E-10 9.2E-09 1E-08 4.33E-09 -1.28E-09 0 0 -1.37E-08
incidence
kBq U235
IR 6.84E-01 3.12E-04 6.25E-02 0 6.78E-02 0 1.75E-05 8.27E-03 1.37E-02 3.91E-03 -2.67E-02 0 0 -6.71E-03
eq
ETP-fw CTUe 7.2E+01 1.2E+00 6.66E+00 3.6E-03 2.69E+00 0 6.73E-02 6.27E-01 8.83E-01 2.11E+00 -4.4E-01 0 0 -4.67E+00
HTP-c CTUh 2.64E-09 2.42E-11 2.44E-10 0 6.21E-10 0 1.36E-12 3.53E-11 4.12E-11 9.48E-11 -2.03E-11 0 0 -5.44E-11
HTP-nc CTUh 8.62E-08 1.44E-09 8.11E-09 2.6E-11 9.46E-09 0 8.07E-11 2.19E-09 2.48E-09 7.94E-09 -7.78E-10 0 0 -3.23E-09
SQP SQP ND ND ND ND ND ND ND ND ND ND ND ND ND ND
PM = Potential incidence of disease due to PM emissions; IR = Potential Human exposure efficiency relative to U235; ETP-fw = Potential comparative
Toxic Unit for ecosystems; HTP-c = Potential comparative Toxic Unit for humans (cancerogenic); HTP-nc = Potential comparative Toxic Unit for humans
(not cancerogenic); SQP = Potential soil quality index
The SQP indicator is not given due to considerable uncertainties in the calculation.
The result figures given in module B2 refer to a period of 1 year because a reference service life is not declared. They have to be
multiplied by the assumed service life (in years) of the floor covering in the building under consideration.
Disclaimer 1 – for the indicator 'Potential Human exposure efficiency relative to U235'.
This impact category deals mainly with the eventual impact of low dose ionizing radiation on human health of the nuclear fuel cycle. It
does not consider effects due to possible nuclear accidents, occupational exposure or radioactive waste disposal in
undergroundfacilities. Potential ionizing radiation from the soil, from radon and from some construction materials is also not measured
by this indicator.
Disclaimer 2 – for the indicators 'abiotic depletion potential for non-fossil resources', 'abiotic depletion potential for fossil resources',
'water (user) deprivation potential, deprivation-weighted water consumption', 'potential comparative toxic unit for ecosystems', 'potential
comparative toxic unit for humans – cancerogenic', 'Potential comparative toxic unit for humans - not cancerogenic', 'potential soil
quality index'.
The results of this environmental impact indicator shall be used with care as the uncertainties on these results are high as there is
limited experienced with the indicator.
References
EN 1307
DIN EN 1307: 2014+A1:2016+A2:2018-05: Textile floor ISO 10874
coverings - Classification DIN EN ISO 10874: 2012+A1:2021-04: Resilient, textile and
laminate floor coverings - Classification
EN 13501-1
DIN EN 13501-1:2019-05: Fire classification of construction ISO 14025
products and building elements - Part 1: Classification using DIN EN /ISO 14025:2011-10/, Environmental labels and
data from reaction to fire tests declarations — Type III environmental declarations —
Principles and procedures
EN 14041
DIN EN 14041: 2018-05 and DIN EN 14041: 2008-05: ISO 14040
Resilient, textile and laminate floor coverings - Essential DIN EN ISO 14040:2006+A1:2020 Environmental
characteristics management - Life cycle assessment - Principles and
framework
EN 15804
DIN EN 15804:2012+A2:2019 + AC:2021, Sustainability of ISO 14044
construction works — Environmental Product Declarations — DIN EN ISO 14044:2006+A1:2018+A2:2020 Environmental
Core rules for the product category of construction products management - Life cycle assessment - Requirements and
guidelines
EN 16810
DIN EN 16810: 2017-08: Resilient, textile and laminate floor ISO 15686
coverings – Environmental product declarations – Product ISO 15686: Buildings and constructed assets - Service life
category rules planning
Environmental Product Declaration - Fletco Carpets A/S - Woven broadloom carpet, pile material solution-dyed polyamide 6.0 with a woven textile or a "Silent Bac"
6 backing, both backings with recycled content, maximum total pile weight 400 g/m²
ISO 15686-1: 2011-05: Part 1: General principles and
framework GaBi database
ISO 15686-2: 2012-05: Part 2: Service life prediction GaBi Software-System and Database for Life Cycle
procedures Engineering, thinkstep AG, Leinfelden-Echterdingen, 2022-2
ISO 15686-7: 2017-04: Part 7: Performance evaluation for
feedback of service life data from practice PCR Part A
ISO 15686-8: 2008-06: Part 8: Reference service life and Product Category Rules for Building-Related Products and
service- Services Part A: Calculation Rules for the Life Cycle
life estimation Assessment and Requirements on the Project Report according
to EN 15804+A2:2019, V1.3, Berlin: Institut Bauen und Umwelt
Regulation (EU) No. 305/2011 e.V. (IBU), August 2022
Regulation No. 305/2011 Construction Products Regulation
(CPR) of the European Council and of the European PCR Part B
Parliament, April 2011 Product Category Rules for Building-Related Products and
Services Part B: Requirements on the EPD for floor coverings,
General Instructions for the IBU-EPD Program V1.3, Berlin: Institut Bauen und Umwelt e.V. (IBU), September
General Instructions for the EPD-Program of the Institut Bauen 2022
und Umwelt e.V., The Preparation of Environmental Product
Declarations - EPDs, version 2.0, Institut Bauen und Umwelt PRODIS
e.V., Berlin, January 2021, www.ibu-epd.de Product Information System (PRODIS) of the European Carpet
Industry, Gemeinschaft umweltfreundlicher Teppichboden e.V
BBSR (GUT) and European Carpet and Rug Association (ECRA),
Bundesinstitut für Bau-, Stadt- und Raumforschung (BBSR) im http://www.pro-dis.info
Bundesamt für Bauwesen und Raumordnung (BBR), Bonn
REACH
BNB, Nutzungsdauer von Bauteilen Regulation (EC) No 1907/2006 of the European Parliament and
Bewertungssystem Nachhaltiges Bauen (BNB), Nutzungsdauer of the Council of 18 December 2006 concerning the
von Bauteilen, Bundesministerium des Inneren, für Bau und Registration, Evaluation, Authorisation and Restriction of
Heimat, 24.02.2017 Chemicals (REACH), June 2017
ECHA candidate list VDZ e.V.
Candidate List of substances of very high concern (SVHCs) for Association of German Cement Works, Ed. Environmental Data
authorisation, last update 26.07.2022, European Chemicals of the German Cement Industry 2020
Agency (ECHA), Helsinki, Finland
Environmental Product Declaration - Fletco Carpets A/S - Woven broadloom carpet, pile material solution-dyed polyamide 6.0 with a woven textile or a "Silent Bac"
7 backing, both backings with recycled content, maximum total pile weight 400 g/m²
Publisher
Institut Bauen und Umwelt e.V. +49 (0)30 3087748- 0
Hegelplatz 1 info@ibu-epd.com
10117 Berlin www.ibu-epd.com
Germany
Programme holder
Institut Bauen und Umwelt e.V. +49 (0)30 3087748- 0
Hegelplatz 1 info@ibu-epd.com
10117 Berlin www.ibu-epd.com
Germany
Author of the Life Cycle Assessment
Gemeinschaft umweltfreundlicher Teppichboden +49 (0)241 96843 410
(GUT) e.V. mail@gut-ev.de
Schönebergstraße 2 www.gut-ev.org
52068 Aachen
Germany
Owner of the Declaration
Fletco Carpets A/S +45 (0)96 60 30 00
Mads Clausens Vej 2 fletco@fletco.dk
7441 Bording www.fletcocarpets.com
Denmark
Environmental Product Declaration - Fletco Carpets A/S - Woven broadloom carpet, pile material solution-dyed polyamide 6.0 with a woven textile or a "Silent Bac"
8 backing, both backings with recycled content, maximum total pile weight 400 g/m²
