ENVIRONMENTAL PRODUCT DECLARATION
as per ISO 14025 and EN 15804+A1
Owner of the Declaration Troldtekt A/S
Programme holder Institut Bauen und Umwelt e.V. (IBU)
Publisher Institut Bauen und Umwelt e.V. (IBU)
Declaration number EPD-TRO-20210107-ICA1-EN
Issue date 27.04.2021
Valid to 26.04.2026
Acoustic panels - painted
Troldtekt A2 Natural Grey
www.ibu-epd.com | https://epd-online.com
Umwelt Produktdeklaration Name des Herstellers – Name des Produkts
1. General Information
Troldtekt A/S A2 Natural Grey, painted
Programme holder Owner of the declaration
IBU – Institut Bauen und Umwelt e.V. Troldtekt A/S
Panoramastr. 1 Sletvej 2 A
10178 Berlin 8310 Tranbjerg
Germany Denmark
Declaration number Declared product / declared unit
EPD-TRO-20210107-ICA1-EN Acoustic panel "A2 Natural Grey" - 1 m2, 25 mm
thickness - painted finish
This declaration is based on the product Scope:
category rules: This declaration represents the production, supply,
Wood cement - Mineral-bonded wooden composites, mounting, use, dismantling and disposal of 1 m2 (25
01.2019 mm thickness) of grey cement-bonded wood wool
(PCR checked and approved by the SVR) acoustic panel "A2 Natural Grey" with a painted
finish, produced by Troldtekt A/S, with a reference
service life of 50 years. The production facility is
Issue date
located in Jutland, Denmark. Three scenarios
27.04.2021
represent its use in indoor conditions in Denmark,
Sweden and Germany.
Valid to
26.04.2026
The owner of the declaration shall be liable for the
underlying information and evidence; the IBU shall not
be liable with respect to manufacturer information, life
cycle assessment data and evidences.
The EPD was created according to the specifications
of EN 15804+A1. In the following, the standard will be
simplified as EN 15804.
Verification
The standard EN 15804 serves as the core PCR
Independent verification of the declaration and data
according to ISO 14025:2010
Dipl. Ing. Hans Peters internally x externally
(chairman of Institut Bauen und Umwelt e.V.)
Dr. Alexander Röder Ms Jane Anderson
(Managing Director Institut Bauen und Umwelt e.V.)) (Independent verifier)
2. Product
2.1 Product description/Product definition 2.2 Application
Troldtekt A2 Natural Grey acoustic panels are some of The panels are installed on the ceilings and walls in
the leading and preferred solutions for creating a good offices, businesses, schools, institutions, cultural sites,
indoor sound environment. They are sold in sports centers, swimming pools and private homes.
various thicknesses (20-35 mm) and dimensions
(width: 600 mm, lengths: 600/1200/2400 mm or width: 2.3 Technical Data
625 mm, lengths: 625/1250/2500 mm). The panels The table below indicates the technical specifications
can be unpainted or painted in a wide variety of of the panels in accordance with EN 13168, the
colors. standard for cement-bonded wood wool and double-
layer panels with cement-bonded wood wool, and EN
For the placing on the market of the product in the 13964, the standard for suspended ceilings.
European Union/European Free Trade Association
(EU/EFTA) (with the exception of Switzerland)
Regulation (EU) No. 305/2011 (CPR) applies. The
product needs a declaration of performance taking into
consideration EN 13964:2014, Suspended ceilings.
Requirements and test methods, and the CE-marking.
For the application and use, the respective national
provisions apply.
2 Environmental Product Declaration Troldtekt A/S – Troldtekt 25mm A2 Natural Grey - painted
Technical specifications of the product covered in 2.8 Product processing/Installation
this EPD Installation instructions are available here:
Name Value Unit https://www.troldtekt.com/Installation
Gross density 523 kg/m3
Grammage 13,06 kg/m2 2.9 Packaging
Thermal conductivity acc. to DIN The product is packaged with plastic film and
76 W/(mK)
52612 cardboard. The packaging material can be easily
Water vapour diffusion resistance sorted and treated in dedicated waste recycling
- -
factor acc. to DIN 4108-4 channels. The packaged product is delivered on a
Sound absorption coefficient (only returnable wood pallet.
with reference to the - %
corresponding component design)
Light reflection (measured by 2.10 Condition of use
DELTA Light and Optics 26,3 - 70,8 % Conditions of use are detailed
Reaction to fire A2/s1/d0 here: https://www.troldtekt.com/Installation/Use_and_
maintenance
2.11 Environment and health during use
Performance data of the product in accordance with
Environmental and ecotoxicity risks from exposure to
the declaration of performance with respect to its
Troldtekt panel products during use have been
essential characteristics according to EN
assessed and found eligible to the following
13168:2012+A1:2015, Thermal insulation products for
certification schemes:
buildings. Factory made wood wool (WW) products.
Specification, and EN 13964:2014, Suspended  Finnish M1 classification
ceilings. Requirements and test methods.  Danish Indoor Climate
2.4 Delivery status
These certificates can be accessed
The panel is usually distributed in length of 600,
here: https://www.troldtekt.com/Web-
1200 or 2400 mm by 600 mm width or in length of 625,
tools/Downloads/Certificates-and-tests
1250 or 2500 mm by 625 mm width. It comes in
three thicknesses: 20, 25 and 35 mm. Additionally,
2.12 Reference service life
several density ranges are available: Coarse, Fine,
The technical service life of the panel is superior to 50
Ultra-Fine and Extreme-Fine causing different
years. This EPD refers to the service lifetime indicated
densities (388-428 kg/m3). The panels are normally
by the BBSR table for the material 353.311 of type
delivered in packs of 80 units on pallets.
“Holzbekleidungen: Holz, Holzwerkstoff und
Mehrschichtleichtbauplatten”.
2.5 Base materials/Ancillary materials
The composition of the finished product is a mix of
Because the panel is used in a building, in this EPD its
limestone (19,1%), wood wool (23,2%), Portland
reference service life is limited by the expected service
cement (53,8%), water (0,6%), as well as water glass
life of the building, which is commonly accepted as 50
(1,0%) and accelerator (1,2%). Additionally, a painted
years, at least as LCA timeframe.
finish is provided with a water-based paint (1,1%). The
composition is at dry basis at the factory gate, as most
There is no influence of the ageing of the material on
of the water has evaporated during drying, but water
its technical performances.
remains bound to the wood fibre and cement paste
(hydrated cement).
2.13 Extraordinary effects
2.6 Manufacture
Fire
Norway spruce logs from local forests (with a moisture
Information on the fire performance according to EN
content of about 65-70%) are received and the bark is
13168.
removed. The wood is stored for approximately six
months until the moisture content in the wood drops to
Fire protection
29%. The wood is then shredded to produce wool. The
Name Value
wood wool is mixed together with Portland cement,
Building material class A2
water, and additives. The mixture is cast and cured
Burning droplets d0
using a heat press and dried with a biomass-fired
Smoke gas development s1
oven. The cast panel is milled to remove any material
in excess and cut edges. After approximately 4 weeks
Water
of curing, the panel can be painted before being stored
No information on the product performance under the
on a pallet and packaged to be transported to central
unforseeable influence of water is available.
distribution warehouses.
Mechanical destruction
2.7 Environment and health during
No information on the product performance under
manufacturing
unforseeable mechanical destruction is available.
Troldtekt is following its working environment closely.
Both the physical working environment and sickness
2.14 Re-use phase
absence are closely monitored. It is an ongoing
Currently, Troldtekt panels undergo thermal treatment
process involving both leaders and factory workers.
with energy recovery. Composting is also possible.
Additional information on recycling
options: https://www.troldtekt.com/~/media/Files/Info%
3 Environmental Product Declaration Troldtekt A/S – Troldtekt 25mm A2 Natural Grey - painted
20sheets/English/Troldtekt_Recycling%20instructions
%20pdf.pdf Additional information on disposal
options: https://www.troldtekt.com/environment-and-
2.15 Disposal csr/product-life-cycle/recycling/
The product may be composted, thermally treated with
energy recovery, or landfilled. 2.16 Further information
For additional information on technical specifications,
European Waste Code: 10 13 11 (wastes from you may consult the Declaration Of
cement-based composite materials) Performance: https://www.troldtekt.com/Web-
tools/Downloads/DoPs
Painted panels must be incinerated at end-of-life.
3. LCA: Calculation rules
3.1 Declared Unit 3.6 Data quality
The functional unit is 1 m2 of acoustic panel, in 25 mm Statistical representativeness
thickness, corresponding to 13,06 kg of material with a The statistical representativeness of the product
painted finish, mounted on ceiling, with a reference system is very good. The input and output data
service life of 50 years. samples used to build inventories are based on the
entirety of the annual production of panels in 2020 and
Declared unit is verified by a third party. Such representativeness is
Name Value Unit also valid for the production of Portland cement, whose
Declared unit 1 m2 EPDs, however, were published in 2021 (white) and
Gross density 523 kg/m3 2017 (grey). The EPD for the paint used was published
Grammage 13.06 kg/m2 in 2018.
conversion factor [Mass/Declared
13.06 -
Unit] Temporal, geographical and technological
Layer thickness 0.025 m representativeness
Environmental impacts for a similar functional unit with All data strictly related to the cement production is
a larger thickness can be approximated using the technologically, temporally, and geographically
following formula: representative. The cement production data is less
than 5 years old. However, since the improvement in
Impact x (New thickness [m] / 0,025 [m]) grey cement production processes in the meantime
have not been accounted for, the LCA results for the
Troldtekt panels based on grey cement can be said to
3.2 System boundary be conservative. The data used to model the
Cradle to grave foreground inventory of acoustic panels dates from the
production year of 2020. As for secondary data, some
3.3 Estimates and assumptions most of the ecoinvent datasets are less than 3 years
Assumptions are described occasionally throughout old.
the section "LCA: Calculation rules".
3.7 Period under review
3.4 Cut-off criteria The primary data concerned with the manufacture (A1-
The cut-off criterion is applied according to EN 15804 A3) relates to the production year 2020 and the data
Section 6.3.5 and PCR part A Section 5.6. are based on the volumes produced on an annual
All inputs and outputs for which data are available are basis.
included in the LCA model. Data gaps are filled with
conservative assumptions from average data (when 3.8 Allocation
available) or with generic data and are documented Allocation of production data to the multiple produced
accordingly. types of panels (with the same functional unit) is
The following product flows have been omitted performed based on the rules provided in EN 15804.
according to the 1% cut-off rule: Sub-processes associated to painting have specially
 Wooden pallet to transport the product been allocated to the painted panels. Data such as
waste generation and packaging have been allocated
 Capital infrastructure (factory)
to the entire production volume of panels in Troldtekt.
 Energy utilization of incinerated paint
The only case of co-produced outputs is associated to
 Allocation of burden from wood logging to wood logging. However, the environmental load is
residual wood fractions evenly distributed over all its co-products, such as
logs, energy wood, and bark.
3.9 Comparability
3.5 Background data
Basically, a comparison or an evaluation of EPD data
Two types of data source are used as secondary data:
is only possible if all the data sets to be compared
 Product-specific EPDs for the manufacture
were created according to EN 15804 and the building
and supply of Portland cement and water- context, respectively the product-specific
based paint characteristics of performance, are taken into account.
 Database ecoinvent v.3.6 cut-off
The used background database is ecoinvent v.3.6 cut-
off
4 Environmental Product Declaration Troldtekt A/S – Troldtekt 25mm A2 Natural Grey - painted
4. LCA: Scenarios and additional technical information
Manufacture (A1-A3)
Data
Primary data is third-party verified and based on the Installation into the building (A5)
production year 2020, within the facilities of Troldtekt Name Value Unit
A/S in Jutland (Denmark). Electricity consumption 0,060 kWh
Material loss (plastic film) 0,007 kg
End-of-waste state and use of by-products Material loss (cardborad) 0,032 kg
For all processes supplying a residual material/waste Use phase (B1)
that originates the end-of-life phase of a product to the Prior to distribution and during the use phase (B1), the
product system to be used as input, the polluter-pay carbonation of the cement contained in the panel,
principle “100:0” is used. Some wooden by-products during use, is accounted for. Based on laboratory
generated during manufacture in Troldtekt end up as measurement, the panel will absorb up to 140 grams of
soil improvers externally (reaching end-of-waste state), carbon dioxide per kilogram of cement. Normalized to
and thus their biogenic carbon leaves Troldtekt's the reference flow, this corresponds to an uptake of
system boundary. approximately 0,9 kilograms of carbon dioxide by the
end of the service lifetime, including the uptake in A3.
Wind-certified electricity
All the electricity used to produce the panels in the Maintenance (B2)
Module A3 originates from Danish wind power, for As the panel does not require any maintenance except
which a certificate ensures the origin. It originates from for the occasional dusting, no maintenance module
a 1-3 MW offshore wind turbine, with transformation, (B2) is considered.
transmission and distribution losses and is modelled
correspondingly. Information about reference service life is detailed in
2.12.
Carbon balance
Biogenic: Absorption of biogenic CO 2 by the purchased Reference service life
wood has been considered in A1. Some of it is Name Value Unit
released again during production in A3, some ends up Reference service life (according to
50 a
sequestered in soil, while the majority of the remaining ISO 15686-1, -2, -7 and -8)
biogenic CO 2, 6,10 kg, is retained in the finished Life Span (according to BBSR) 50 a
product and emitted during end-of-life incineration in Life Span according to the
C4. manufacturer 75 a
Fossil: Absorption of some fossil CO 2, originating from
the calcination of limestone during cement production, End of life (C1-C4)
happens when the cement is mixed with water in A3. A
Name Value Unit
majority is absorbed during the use phase B1, and all Electricity use (for un-mounting) 0,060 kWh
the absorbed fossil CO is finally emitted during end-
2 Transport (to material sorting facility) 50 km
of-life incineration in C4.
Collected as mixed construction waste 13,06 kg
Energy recovery 2,99 kg
Distribution to site (A4) and mounting (A5)
Energy recovery efficiency 10 %
To consider the main geographical variants of the life
Energy recovered 6,10 MJ
cycle of Troldtekt A2 Natural Grey panels, three
scenarios are developed, where the product is
The panel is un-mounted at the end of its reference
supplied, mounted, used and discarded in Aarhus
service life and driven to the regional waste
(Denmark), Hamburg (Germany) and Malmö
incineration plant. Energy is recovered from the wood
(Sweden). An additional 50 km from the local
part of the panel at 10% efficiency.
warehouse to construction site is assumed.
Transport to the building site (A4) Reuse, recovery and/or recycling potentials (D),
Name Value Unit relevant scenario information
Litres of fuel 26,8 l/100km Name Value Unit
Transport distance to Denmark 160 km Electricity 1,45 MJ
Transport distance to Germany 370 km Heat 4,65 MJ
Transport distance to Sweden 394 km
Transport distance from The energy substituted from incineration of the panel's
warehouse to local construction wood component in C4 is considered being a split of
50 km
sites in the Danish electricity grid mix (for electricity) and
Denmark/Germany/Sweden natural gas (for heat).
Capacity utilisation (including
empty runs) 85 % Details on possible disposal routes
Aalborg Portland cement factory utilizes dust and
Gross density of products
471 kg/m3 offcuts from the Troldtekt factory as a raw material in
transported
new cement, i.e. in the technical circle. During
Capacity utilisation volume factor 1 -
incineration in the cement kiln, the wood content in the
cement bonded wood wool panels replaces fossil fuels,
5 Environmental Product Declaration Troldtekt A/S – Troldtekt 25mm A2 Natural Grey - painted
while the cement ends up as a raw material in new
cement, replacing virgin raw materials and heavy fossil
fuels, thereby avoiding a significant amount of CO
2
emissions. This scheme of wood wool waste as a raw
material can be scaled for construction site and
demolition waste. It will be gradually rolled out to all of
Denmark in the period 2021-2023. Once Denmark has
documented economic and environmental benefits to
be gained by including wood wool waste in the
production of new cement rather than going to waste
incineration or landfill, dialogue with municipalities and
local cement producers in the primary markets of
Troldtekt is initiated to facilitate similar schemes
regionally or nationally.
6 Environmental Product Declaration Troldtekt A/S – Troldtekt 25mm A2 Natural Grey - painted
5. LCA: Results
Note: Global Warming Potential (GWP) indicator includes CO of both biogenic and fossil origin.
2
Also, GWP results for Troldtekt A2 Natural Grey (painted) for other delivery scenarios in respectively Germany
and Sweden, are 2,58E-1 kg CO and 2,73E-1 kg CO .
2 2
DESCRIPTION OF THE SYSTEM BOUNDARY (X = INCLUDED IN LCA; MND = MODULE NOT DECLARED;
MNR = MODULE NOT RELEVANT)
BENEFITS AND
CONSTRUCTI LOADS
PRODUCT STAGE ON PROCESS USE STAGE END OF LIFE STAGE BEYOND THE
STAGE SYSTEM
BOUNDARIES
7 Environmental Product Declaration Troldtekt A/S – Troldtekt 25mm A2 Natural Grey - painted
lairetam
waR
ylppus tropsnarT
gnirutcafunaM
eht
morf
tropsnarT
etis
eht
ot
etag
ylbmessA esU
ecnanetniaM
riapeR
tnemecalpeR tnemhsibrufeR
ygrene
lanoitarepO esu
retaw
lanoitarepO esu
noitcurtsnoc-eD
noitilomed tropsnarT
gnissecorp
etsaW
lasopsiD -esueR -yrevoceR -gnilcyceR laitnetop
A1 A2 A3 A4 A5 B1 B2 B3 B4 B5 B6 B7 C1 C2 C3 C4 D
X X X X X X MND MNR MNR MNR MND MND X X MND X X
RESULTS OF THE LCA - ENVIRONMENTAL IMPACT according to EN 15804+A1: 1 m2 A2 Natural Grey, 25
mm, painted finish, delivered and used in Denmark
Parameter Unit A1-A3 A4 A5 B1 C1 C2 C4 D
GWP [kg CO2-Eq.] 2.34E+0 1.29E-1 8.76E-2 -7.63E-1 6.50E-4 1.09E-1 7.11E+0 -7.98E-1
ODP [kg CFC11-Eq.] 3.06E-7 2.35E-8 1.64E-9 0.00E+0 2.81E-10 1.99E-8 5.36E-9 -4.41E-8
AP [kg SO2-Eq.] 2.09E-2 2.61E-4 5.90E-5 0.00E+0 1.59E-6 2.20E-4 4.43E-4 -1.66E-3
EP [kg (PO4)3--Eq.] 6.93E-3 5.36E-5 1.03E-4 0.00E+0 8.86E-7 4.53E-5 1.92E-4 -1.23E-3
POCP [kg ethene-Eq.] 1.03E-3 1.72E-5 2.58E-6 0.00E+0 8.88E-8 1.45E-5 3.47E-5 -9.52E-5
ADPE [kg Sb-Eq.] 5.83E-5 3.52E-6 2.09E-7 0.00E+0 1.82E-8 2.97E-6 5.84E-7 -2.14E-6
ADPF [MJ] 5.59E+1 1.94E+0 2.93E-1 0.00E+0 4.76E-3 1.64E+0 4.26E-1 -1.29E+1
GWP = Global warming potential; ODP = Depletion potential of the stratospheric ozone layer; AP = Acidification potential of land and water; EP =
Caption Eutrophication potential; POCP = Formation potential of tropospheric ozone photochemical oxidants; ADPE = Abiotic depletion potential for non-
fossil resources; ADPF = Abiotic depletion potential for fossil resources
RESULTS OF THE LCA - INDICATORS TO DESCRIBE RESOURCE USE according to EN 15804+A1: 1 m2
A2 Natural Grey, 25 mm, painted finish, delivered and used in Denmark
Parameter Unit A1-A3 A4 A5 B1 C1 C2 C4 D
PERE [MJ] 6.05E+1 2.77E-2 1.60E-1 0.00E+0 3.91E-2 2.34E-2 7.06E+0 -5.22E+0
PERM [MJ] 6.15E+1 0.00E+0 0.00E+0 0.00E+0 0.00E+0 0.00E+0 0.00E+0 0.00E+0
PERT [MJ] 1.22E+2 2.77E-2 1.60E-1 0.00E+0 3.91E-2 2.34E-2 7.06E+0 -5.22E+0
PENRE [MJ] 5.79E+1 1.98E+0 4.58E-1 0.00E+0 4.31E-2 1.67E+0 5.58E-1 -1.41E+1
PENRM [MJ] 1.51E-1 0.00E+0 0.00E+0 0.00E+0 0.00E+0 0.00E+0 0.00E+0 0.00E+0
PENRT [MJ] 5.81E+1 1.98E+0 4.58E-1 0.00E+0 4.31E-2 1.67E+0 5.58E-1 -1.41E+1
SM [kg] 2.26E+0 0.00E+0 3.10E-2 0.00E+0 0.00E+0 0.00E+0 0.00E+0 0.00E+0
RSF [MJ] 5.13E+0 0.00E+0 0.00E+0 0.00E+0 0.00E+0 0.00E+0 0.00E+0 0.00E+0
NRSF [MJ] 5.73E+0 0.00E+0 0.00E+0 0.00E+0 0.00E+0 0.00E+0 0.00E+0 0.00E+0
FW [m³] 5.55E-1 3.36E-4 1.30E-4 0.00E+0 1.19E-5 2.83E-4 2.35E-4 -1.53E-3
PERE = Use of renewable primary energy excluding renewable primary energy resources used as raw materials; PERM = Use of
renewable primary energy resources used as raw materials; PERT = Total use of renewable primary energy resources; PENRE = Use of
non-renewable primary energy excluding non-renewable primary energy resources used as raw materials; PENRM = Use of non-
Caption
renewable primary energy resources used as raw materials; PENRT = Total use of non-renewable primary energy resources; SM = Use
of secondary material; RSF = Use of renewable secondary fuels; NRSF = Use of non-renewable secondary fuels; FW = Use of net fresh
water
RESULTS OF THE LCA – WASTE CATEGORIES AND OUTPUT FLOWS according to EN 15804+A1:
1 m2 A2 Natural Grey, 25 mm, painted finish, delivered and used in Denmark
Parameter Unit A1-A3 A4 A5 B1 C1 C2 C4 D
HWD [kg] 6.47E-2 1.99E-3 1.51E-3 0.00E+0 5.40E-5 0.00E+0 1.24E-3 -4.88E-2
NHWD [kg] 1.97E+0 1.37E-1 1.15E-1 0.00E+0 1.12E-3 0.00E+0 5.18E-2 -1.66E+0
RWD [kg] 1.14E-4 1.35E-5 2.54E-6 0.00E+0 5.78E-7 0.00E+0 4.16E-6 -2.02E-5
CRU [kg] 6.83E-6 0.00E+0 0.00E+0 0.00E+0 0.00E+0 0.00E+0 0.00E+0 0.00E+0
MFR [kg] 1.62E-2 0.00E+0 0.00E+0 0.00E+0 0.00E+0 0.00E+0 0.00E+0 0.00E+0
MER [kg] 8.99E-3 0.00E+0 0.00E+0 0.00E+0 0.00E+0 0.00E+0 0.00E+0 0.00E+0
EEE [MJ] 0.00E+0 0.00E+0 0.00E+0 0.00E+0 0.00E+0 0.00E+0 1.45E+0 0.00E+0
EET [MJ] 0.00E+0 0.00E+0 0.00E+0 0.00E+0 0.00E+0 0.00E+0 4.65E+0 0.00E+0
HWD = Hazardous waste disposed; NHWD = Non-hazardous waste disposed; RWD = Radioactive waste disposed; CRU = Components
Caption for re-use; MFR = Materials for recycling; MER = Materials for energy recovery; EEE = Exported electrical energy; EEE = Exported
thermal energy
6. LCA: Interpretation
The estimated impact results are only relative acquisition and use of cement, wood, and paint in the
statements which do not indicate the end points of the foreground processes. Global Warming Potential net
impact categories, exceeding threshold values, safety emissions share is much larger in C4 than in A1-A3
margins or risks. (see why in chart (2)), while other impact categories in
module D in general are avoided in the waste system
Two charts are presented: (1) with the standard owing to the incineration of end-of-life panels and
lifecycle impact categories displaying the share of substitution of natural gas and Danish electricity mix.
impacts across all lifecycle stages, and (2) displaying C4 also slightly follows emissions of compounds
the total carbon balance of the Troldekt product's associated to other impact categories. A relatively
lifecycle system. inefficient transportation of end-of-life panels to waste
incineration causes emissions in especially Abiotic
Impacts from the A1-A3 modules are dominant in the depletion of non-fossil resources, Depletion of
life cycle of the Troldtekt A2 Natural Grey painted stratospheric ozone, and Photochemical ozone
panel products. This is primarily caused by the formation.
The embodied emissions associated to the raw sequestered in A1-A3 and some fossil CO taken up in
2
materials (primarily cement and paint) are the main A1-A3 and B1 is re-emitted in C4. CO emissions
2-eq
cause of impacts, especially in terms of net Global occuring in the remaining modules are negligible.
Warming Potential, with respectively 7,2 kg CO and
2-eq
0,4 kg CO followed by minor impacts from additives. The amount of wood stored in the product refers to a
2-eq
In general, direct emissions from the Troldtekt negative contribution to Global Warming Potential,
production site are relatively small. Abiotic depletion of reducing the share of Global Warming Potential in A1-
fossil resources appears from the burden of producing A3. This is due to the sequestration of biogenic carbon
cement using fossil raw material such as limestone of wood during tree growth. The sequestered carbon
and to a large extent fossil fuels. In terms of carbon does not contribute to global warming as long as it is
balance, biogenic CO in A1-A3 offsets nearly all the stored in the biomass.
2
fossil CO emissions in A1-A3. All biogenic CO
2 2
8 Environmental Product Declaration Troldtekt A/S – Troldtekt 25mm A2 Natural Grey - painted
Summary Global Warming and Eutrophication, by order of
Within the cradle to grave, the following aspects have importance. The treatment of wastewater from the
been identified as major contributors, mainly in the painting cabin also contributes significantly to potential
categories Global Warming Potential and Abiotic impacts in terms of Eutrophication.
depletion of fossil resources:
The clinker (cement) production is the most critical
 Emissions from the clinker production from process of the Troldtekt product system, but
material inaccuracies around the amount used will not
invalidate the present conclusions.
 Emissions from the clinker production from
fuel
Notably, by introducing more up-to-date LCA datasets
 Substituted emissions from end of life for the grey cement applied, or introducing cements
incineration with less carbon footprint into production, as well as
improved paint consumption management, could lead
to significant reductions of especially the Global
Additionally, for painted panels, the manufacture of
Warming Potential indicator.
paint contribute significantly to impacts on potentials
for Photochemical ozone formation, Acidification,
7. Requisite evidence
7.3 VOC emissions
7.1 Testing of substances used Testing for VOC emissions has been conducted in
A detailed assessment of substances used was accordance with EN ISO 16000-6. Analysis of the air
conducted by a DAkkS-accredited laboratory, based sampled on Tenax was performed at the Danish
on a sample (prepared according to EN 15443), Technological Institute under DANAK accreditation
available in the Test Report 2018P216294, using 392. Report no. MAIC-2019-1418. Reporting of
inductively coupled plasma mass spectrometry (EN measured concentrations in toluene equivalents
16171) and X-ray fluorescence (EN 15309), for the according to EN 16516. This test is basis for the Finish
following: M1 Material certificate as well as the Danish Indoor
 Heavy metals (cadmium, mercury, etc.) Climate labeling certificate.
 and other elements
AgBB overview of results (28 days [µg/m³])
Name Value Unit
7.2 Leaching TVOC (C6 - C16) 12 μg/m3
No leaching measurement was conducted according to Sum SVOC (C16 - C22) 0 - 5 μg/m3
EN 717-1. VOC without NIK 0 - 5 μg/m3
Carcinogenic Substances 1 μg/m3
8. References
Standards DIN EN ISO 14025
DIN EN ISO 14025:2011, Environmental labels and
AgBB declarations – Type III environmental
AgBB, Ausschuss zur gesundheitlichen Bewertung von declarations – Principles and procedures, German and
Bauprodukten (Committee for Health-related English versions EN ISO 14025:2011
Evaluation of Building Products)
EN 13168
BBSR EN 13168:2012+A1:2015, Thermal insulation products
BBSR, Bundesinstitut für Bau-, Stadt- und for buildings. Factory made wood wool (WW) products.
Raumforschung (Federal Institute for Research on Specification
Building, Urban Affairs and Spatial Development).
BBSR table: EN 13964
https://www.nachhaltigesbauen.de/fileadmin/pdf/baust EN 13964:2014, Suspended ceilings. Requirements
off_gebauededaten/BNB_Nutzungsdauern_von_Bautei and test methods
len_2017-02-24.pdf
EN 15309
DIN 4108-4 EN 15309:2007, Characterization of waste and soil.
DIN 4108-4:2017-03, Thermal insulation and energy Determination of elemental composition by X-ray
economy in buildings - Part 4: Hygrothermal design fluorescence
values
EN 15443
DIN 52612-2 EN 15443:2011, Solid recovered fuels. Methods for the
DIN 52612-2, Testing of thermal insulating materials; preparation of the laboratory sample
determination of thermal conductivity by means of the
guarded hot plate apparatus; conversion of the EN 15804
measured values for building applications. 1 June 1984 EN 15804:2012, EN 15804:2012+A1 2013,
Sustainability of construction works – Environmental
9 Environmental Product Declaration Troldtekt A/S – Troldtekt 25mm A2 Natural Grey - painted
Product Declarations – Core rules for the product
category of construction products. Product Category Rule A
Product Category Rule A, IBU, 2019, Part A,
EN 16171 Calculation Rules for the Life Cycle Assessment and
EN 16171:2016, Sludge, treated biowaste and soil. Requirements on the Project Report. v.1.8. IBU, 2019.
Determination of elements using inductively coupled
plasma mass spectrometry (ICP-MS) Product Category Rule B
Product Category Rule B, IBU, 2019, Part B,
EN 16449 Requirements on the EPD for Wood cement - Mineral-
EN 16449:2014, EN 16449:2014, Wood and wood- bonded wooden composites. v.1.7. IBU, 2019.
based products - Calculation of the biogenic carbon
content of wood and conversion to carbon dioxide
Further References
EN 16516
EN 16516:2017+A1:2020, Construction products: General Programme Instructions, IBU 2016
Assessment of release of dangerous substances. General Programme Instructions for the Preparation of
Determination of emissions into indoor air EPDs at the Institut Bauen und Umwelt e.V. Version 1.,
Berlin: Institut Bauen und Umwelt e.V., 2016.
EN 717-1
EN 717-1:2004, Wood-based Panels – Determination Software/database
of Formaldehyde Release – Formaldehyde emission OneClick LCA software, Pre-verified EPD tool,
by the chamber method Bionova: https://www.oneclicklca.com/
ISO 16000-6 Database: Ecoinvent v.3.6. cut-off (2019)
ISO 16000-6:2011, Indoor air - Part 6: Determination of
volatile organic compounds in indoor and test chamber
air by active sampling on Tenax TA sorbent, thermal
desorption and gas chromatography using MS or MS-
FID
10 Environmental Product Declaration Troldtekt A/S – Troldtekt 25mm A2 Natural Grey - painted
Publisher
Institut Bauen und Umwelt e.V. Tel +49 (0)30 3087748- 0
Panoramastr. 1 Fax +49 (0)30 3087748- 29
10178 Berlin Mail info@ibu-epd.com
Germany Web www.ibu-epd.com
Programme holder
Institut Bauen und Umwelt e.V. Tel +49 (0)30 - 3087748- 0
Panoramastr 1 Fax +49 (0)30 – 3087748 - 29
10178 Berlin Mail info@ibu-epd.com
Germany Web www.ibu-epd.com
Author of the Life Cycle
Assessment Tel 98777223
Aalborg Portland Fax 80815733
Rørdalsvej 44 Mail
92200 Aalborg Ø stefan.e.danielsson@cementirhol
Denmark ding.it
Web www.aalborgportland.dk
Owner of the Declaration
Troldtekt A/S Tel +45 8747 8100
Sletvej 2A Fax +45 8747 8111
8310 Tranbjerg J Mail sales@troldtekt.dk
Denmark Web https://www.troldtekt.com
