ENVIRONMENTAL PRODUCT DECLARATION
as per ISO 14025 and EN 15804+A2
Owner of the Declaration Sika Australia Pty Ltd
Publisher Institut Bauen und Umwelt e.V. (IBU)
Programme holder Institut Bauen und Umwelt e.V. (IBU)
Declaration number EPD-SIK-20240239-CBA2-EN
Issue date 22/07/2024
Valid to 21/07/2029
Sika® Set Accelerator
Sika Australia Pty Ltd
www.ibu-epd.com | https://epd-online.com
General Information
Sika Australia Pty Ltd Sika® Set Accelerator
Programme holder Owner of the declaration
IBU – Institut Bauen und Umwelt e.V. Sika Australia Pty Ltd
Hegelplatz 1 Elizabeth Street 55
10117 Berlin 2164 Wetherill Park, NSW
Germany Australia
Declaration number Declared product / declared unit
EPD-SIK-20240239-CBA2-EN 1 kg of Sika® Set Accelerator with a density of 1.33 kg/l.
This declaration is based on the product category rules: Scope:
Concrete admixtures, 01/08/2021 This verified EPD relates to 1kg of Sika® Set Accelerator. It is
(PCR checked and approved by the SVR) manufactured at the plants of Sika Australia Pty Ltd in Wetherill Park (NSW
2164), Keysborough (VIC 3173), Pinkenba (QLD 4008), and Bibra Lake
(WA 6163) in Australia. The production and transport data are
Issue date representative for the period from July 2022 to June 2023. The results in
this EPD are calculated using an LCA-tool verified by IBU in 2023.
22/07/2024
The owner of the declaration shall be liable for the underlying information
and evidence; the IBU shall not be liable with respect to manufacturer
Valid to
information, life cycle assessment data and evidences.
21/07/2029
The EPD was created according to the specifications of EN 15804+A2. In
the following, the standard will be simplified as EN 15804.
Verification
The standard EN 15804 serves as the core PCR
Independent verification of the declaration and data according to ISO
14025:2011
internally X externally
Dipl.-Ing. Hans Peters
(Chairman of Institut Bauen und Umwelt e.V.)
Florian Pronold Matthias Schulz,
(Managing Director Institut Bauen und Umwelt e.V.) (Independent verifier)
1 Environmental Product Declaration - Sika Australia Pty Ltd - Sika® Set Accelerator
Product
Additional technical data are not relevant for this product.
Product description/Product definition
Sika® Set Accelerator is produced from specially-selected salt Base materials/Ancillary materials
compounds and additives. The admixture is a liquid agent that The raw materials and additives of Sika® Set Accelerator can
is introduced into concrete while it is being mixed. Depending be given as follows:
on specific application, the typical dosage can range from 1000 Name Value Unit
ml to 2000 ml per 100 kg of total cementitious materials.
Selected salt compounds (*) 20–50 %
Optimum dosage should be determined by site trials with the
Water 40–70 %
particular concrete mix design and materials. Users shall refer
to the most recent Product Data Sheet for more information and Additives < 10 %
advice. (*) Solid
Sika® Set Accelerator is accompanied by a declaration of
With respect to international and local regulations:
performance, which conforms to the specifications outlined in
• This product/article/at least one partial article contains
Australian Standard AS 1478.1-2000, type Ac. The product is
substances listed in the 'Candidate List of Substances of
designed to accelerate the setting and increase the early
Very High Concern (SVHC) for Authorisation' (date:
strength of concrete. It can be used for various applications
30/05/2024) exceeding 0.1 percentage by mass: No.
when there are requirements of early strength, faster finishing
• Biocide products were added to this construction
of concrete surfaces, and faster slip-form movement or in case
product or it has been treated with biocide products (this
of cold climate.
then concerns a treated product as defined by the (EU)
Application Ordinance on Biocide Products No. 528/2012): No.
Sika® Set Accelerator is used as a constituent material to • Any applicable prohibition, authorisation and restricted
produce concrete. It can be used in combination with other Sika use requirements for this product, including for
admixtures. All admixtures must be added separately and trials carcinogens referred to in Schedule 10 of the Australian
are recommended before use. Model Work Health and Safety Regulations (WHS): No.
Technical Data
Reference service life
Sika® Set Accelerator meets the requirements of AS 1478.1-
2000, type Ac. The durability of concrete admixtures is normally at least as
long as the lifetime of the building in which it is used. The
Constructional data
experimental data show that the reference life is greater than
Name Value Unit 50 years. The documentation of the Reference service life is
pH of admixture (AS 1478.1) 7.0–9.0 - not required for the EPDs calculated using the EPD tool from
1.31– Sika since the entire life cycle is not declared. Only modules
Relative density of admixture (AS 1478.1) kg/l
1.35 A1-A3, A4, A5, C1, C2, C4, and D are considered.
33.0–
Non-volatile content of admixture (AS 1478.1) %
37.0
Chloride content of admixture (AS 1478.1) ≤ 350 g/l
Water content of concrete as % of control (AS
≤ 105 %
1478.1)
Intial setting time of concrete, deviation from
-3 to -1 hour
control (AS 1012.18)
Final setting time of concrete, deviation from
-3 to -1 hour
control (AS 1012.18)
Compressive strength of concrete as % of
≥ 100 %
control at 3 days (AS 1012.9)
Compressive strength of concrete as % of
≥ 100 %
control at 7 days (AS 1012.9)
Compressive strength of concrete as % of
≥ 100 %
control at 28 days (AS 1012.9)
Compressive strength of concrete as % of
≥ 90 %
control at 90 days (AS 1012.9)
LCA: Calculation rules
Name Value Unit
Declared Unit
Declared unit 1 kg
The EPD refers to the declared unit of 1kg of concrete
admixture applied into the building with a density of 1.33 g/ml in
Gross density 1330 kg/m3
accordance with IBU PCR 04-2023 Part B for concrete Other declared units are allowed if the conversion is shown
admixtures. transparently.
Declared unit and mass reference
System boundary
2 Environmental Product Declaration - Sika Australia Pty Ltd - Sika® Set Accelerator
Declaration type with respect to life cycle stages covered One scenario is considered for the final treatment of the waste:
according to clause 5.2 EN 15804+A2 is cradle to gate with
• 100% disposal (C4), modelled by landfill process where
modules C1–C4 and module D (A1–A3, A4, A5, C and D).
admixtures end their life cycle.
Modules taken into account:
Module D accounts for benefits that are beyond the defined
• A1 Production of preliminary products system boundaries. Credits are generated during the
• A2 Transport to the plant incineration of the installation scrap in module A5.
• A3 Production including provision of energy, production
of auxiliaries and consumables and waste treatment
• A4 Transport from the construction site to the installation Geographic Representativeness
site Land or region, in which the declared product system is
• A5 Installation, admixtures applied into the building manufactured, used or handled at the end of the product´s
during A5 phase operations. At this stage, an impact of lifespan: Australia
the production and treatment of installation residue
equal to 1% of the product is considered.
Comparability
• C1-C2-C4-D
Basically, a comparison or an evaluation of EPD data is only
The building deconstruction (demolition process) takes place in
possible if all the data sets to be compared were created
C1 module which considers energy production and
according to EN 15804 and the building context, respectively
consumption in terms of diesel and all the emissions connected
the product-specific characteristics of performance, are taken
with the fuel-burning process. After the demolition, the
into account. Sphera LCA for Expert software (former GaBi)
admixture is transported to the end-of-life processing (C2
(version 10) and Managed LCA Content (2022.2) have been
module) where all the impacts related to the transport
used.
processes are considered.
LCA: Scenarios and additional technical information
Name Value Unit
Characteristic product properties of biogenic carbon
Material loss 0.01 kg
No biogenic carbon containing material was intended to be
Other resources - kg
used in the product and accompanying packaging.
Material loss regards the amount of product not used during the
Information on describing the biogenic carbon content at application phase into the building. This amount is 1% of the
factory gate product, impacts related to the production of this part are
charged to the A5 module. This percentage is considered as
Name ValueUnit
waste to incineration since the product has a calorific value and
Biogenic carbon content in product - kg impacts of its end of life have been considered in the LCA
C model and declared in A5.
Biogenic carbon content in accompanying kg
-
packaging C
End of life (C1-C4)
Note: 1 kg of biogenic carbon is equivalent to 44/12 kg of CO 2. C1: This module considers the use of machinery (7.5E-5 kg of
diesel for kg handled) to dismantle the product to enable its
subsequent transport.
C2: The concrete demolition waste is transported from the
building site to a treatment plant or disposal site by truck and
Transport from the gate to the site (A4)
an average distance of 50 km is considered.
Name Value Unit
C4: The results for the end-of-life are declared for one scenario:
Transport distance 99 km
Name Value Unit
Gross weight 34–40 t
Landfill percentage 100 %
Payload capacity 27 t
Material to landfill 1 kg
Assembly (A5)
3 Environmental Product Declaration - Sika Australia Pty Ltd - Sika® Set Accelerator
LCA: Results
DESCRIPTION OF THE SYSTEM BOUNDARY (X = INCLUDED IN LCA; MND = MODULE OR INDICATOR NOT DECLARED; MNR
= MODULE NOT RELEVANT)
Benefits and
Construction loads beyond
Product stage Use stage End of life stage
process stage the system
boundaries
la ire ta m w a Ry lp p u s tro p s n a rT g n iru tc a fu n a M e h t m o rf tro p s n a rTe tis e h t o t e ta g y lb m e s s A e s U e c n a n e tn ia M ria p e R tn e m e c a lp e R tn e m h s ib ru fe R y g re n e la n o ita re p Oe s u re ta w la n o ita re p Oe s u n o itc u rts n o c -e Dn o itilo m e d tro p s n a rT g n is s e c o rp e ts a W la s o p s iD -e s u e R-y re v o c e R-g n ilc y c e Rla itn e to p
A1 A2 A3 A4 A5 B1 B2 B3 B4 B5 B6 B7 C1 C2 C3 C4 D
X X X X X MND MND MNR MNR MNR MND MND X X MND X X
RESULTS OF THE LCA - ENVIRONMENTAL IMPACT according to EN 15804+A2: 1 kg Sika® Set Accelerator
Parameter Unit A1-A3 A4 A5 C1 C2 C4 D
GWP-total kg CO 2 eq 2.12E-01 4.95E-03 1.4E-02 2.82E-04 6.27E-03 4.33E-02 -5.46E-03
GWP-fossil kg CO 2 eq 2.09E-01 4.74E-03 8.26E-03 2.7E-04 6E-03 4.29E-02 -5.46E-03
GWP-biogenic kg CO 2 eq 3.7E-03 2.1E-04 5.76E-03 1.21E-05 2.65E-04 4.41E-04 8.95E-07
GWP-luluc kg CO 2 eq 1.29E-05 1.24E-07 1.99E-07 7.16E-09 1.56E-07 1.53E-05 -2.59E-06
ODP kg CFC11 eq 2.72E-13 4.65E-16 3.38E-15 2.69E-17 5.88E-16 6.67E-14 -1.85E-14
AP mol H+ eq 1.57E-03 1.45E-05 2.24E-05 3.66E-06 2E-05 2.12E-04 -1.78E-05
EP-freshwater kg P eq 1.16E-06 5.99E-10 1.2E-08 3.47E-11 7.56E-10 1.33E-07 -1.86E-09
EP-marine kg N eq 4.28E-04 6.47E-06 6.81E-06 1.65E-06 9.02E-06 5.73E-05 -3.93E-06
EP-terrestrial mol N eq 4.72E-03 7.11E-05 7.88E-05 1.81E-05 9.93E-05 6.3E-04 -4.28E-05
kg NMVOC
POCP 1.19E-03 1.31E-05 1.85E-05 4.96E-06 1.8E-05 1.57E-04 -1.17E-05
eq
ADPE kg Sb eq 4.52E-08 1.92E-10 5.27E-10 1.11E-11 2.43E-10 1.14E-08 -3.32E-10
ADPF MJ 3.37E+00 6.56E-02 4.04E-02 3.8E-03 8.29E-02 6.22E-01 -5.87E-02
m3 world eq
WDP 5.31E-02 4.04E-05 1.83E-03 2.34E-06 5.1E-05 2.6E-03 -1.53E-03
deprived
GWP = Global warming potential; ODP = Depletion potential of the stratospheric ozone layer; AP = Acidification potential of land and water; EP =
Eutrophication potential; POCP = Formation potential of tropospheric ozone photochemical oxidants; ADPE = Abiotic depletion potential for non-fossil
resources; ADPF = Abiotic depletion potential for fossil resources; WDP = Water (user) deprivation potential)
RESULTS OF THE LCA - INDICATORS TO DESCRIBE RESOURCE USE according to EN 15804+A2: 1 kg Sika® Set Accelerator
Parameter Unit A1-A3 A4 A5 C1 C2 C4 D
PERE MJ 2.16E-01 3.55E-04 2.65E-03 2.06E-05 4.49E-04 6.01E-02 -1.31E-02
PERM MJ 0 0 0 0 0 0 0
PERT MJ 2.16E-01 3.55E-04 2.65E-03 2.06E-05 4.49E-04 6.01E-02 -1.31E-02
PENRE MJ 1.96E+00 6.57E-02 5.54E-02 3.8E-03 8.3E-02 6.41E-01 -5.87E-02
PENRM MJ 1.43E+00 0 -1.48E-02 0 0 0 0
PENRT MJ 3.4E+00 6.57E-02 4.07E-02 3.8E-03 8.3E-02 6.41E-01 -5.87E-02
SM kg 0 0 0 0 0 0 0
RSF MJ 0 0 0 0 0 0 0
NRSF MJ 0 0 0 0 0 0 0
FW m3 1.3E-03 1.02E-06 4.31E-05 5.89E-08 1.29E-06 9.2E-05 -3.64E-05
PERE = Use of renewable primary energy excluding renewable primary energy resources used as raw materials; PERM = Use of renewable primary
energy resources used as raw materials; PERT = Total use of renewable primary energy resources; PENRE = Use of non-renewable primary energy
excluding non-renewable primary energy resources used as raw materials; PENRM = Use of non-renewable primary energy resources used as raw
materials; PENRT = Total use of non-renewable primary energy resources; SM = Use of secondary material; RSF = Use of renewable secondary fuels;
NRSF = Use of non-renewable secondary fuels; FW = Use of net fresh water
RESULTS OF THE LCA – WASTE CATEGORIES AND OUTPUT FLOWS according to EN 15804+A2:
1 kg Sika® Set Accelerator
Parameter Unit A1-A3 A4 A5 C1 C2 C4 D
HWD kg 2.29E-10 1.65E-13 2.64E-12 9.52E-15 2.08E-13 2.4E-11 -5.45E-12
NHWD kg 5.74E-03 2.72E-06 1.88E-03 1.58E-07 3.44E-06 1E+00 -2.47E-05
RWD kg 7.44E-05 3.7E-08 9.16E-07 2.14E-09 4.67E-08 5.63E-06 -1.1E-06
CRU kg 0 0 0 0 0 0 0
MFR kg 0 0 0 0 0 0 0
MER kg 0 0 0 0 0 0 0
EEE MJ 0 0 2.21E-02 0 0 0 0
EET MJ 0 0 6.23E-03 0 0 0 0
HWD = Hazardous waste disposed; NHWD = Non-hazardous waste disposed; RWD = Radioactive waste disposed; CRU = Components for re-use;
MFR = Materials for recycling; MER = Materials for energy recovery; EEE = Exported electrical energy; EET = Exported thermal energy
4 Environmental Product Declaration - Sika Australia Pty Ltd - Sika® Set Accelerator
RESULTS OF THE LCA – additional impact categories according to EN 15804+A2-optional:
1 kg Sika® Set Accelerator
Parameter Unit A1-A3 A4 A5 C1 C2 C4 D
Disease
PM 2.48E-08 8.04E-11 2.87E-10 1.93E-10 1.08E-10 2.21E-09 -2.44E-10
incidence
IR kBq U235 eq 6.22E-03 2.45E-06 7.68E-05 1.42E-07 3.1E-06 5.17E-04 -6.87E-05
ETP-fw CTUe 2.84E+00 7.77E-02 3.23E-02 4.5E-03 9.82E-02 3.47E-01 -1.06E-02
HTP-c CTUh 1.12E-10 1.25E-12 1.73E-12 7.22E-14 1.58E-12 3.35E-11 -1.01E-12
HTP-nc CTUh 1.1E-08 4.28E-11 1.75E-10 3.5E-12 5.47E-11 3.51E-09 -2.62E-11
SQP SQP 1.34E-01 1.94E-04 2.13E-03 1.12E-05 2.45E-04 7.32E-02 -5.63E-03
PM = Potential incidence of disease due to PM emissions; IR = Potential Human exposure efficiency relative to U235; ETP-fw = Potential comparative
Toxic Unit for ecosystems; HTP-c = Potential comparative Toxic Unit for humans (cancerogenic); HTP-nc = Potential comparative Toxic Unit for humans
(not cancerogenic); SQP = Potential soil quality index
Disclaimer 1 – for the indicator 'Potential Human exposure efficiency relative to U235'. This impact category deals mainly with the
eventual impact of low-dose ionizing radiation on human health of the nuclear fuel cycle. It does not consider effects due to possible
nuclear accidents, occupational exposure or radioactive waste disposal in underground facilities. Potential ionizing radiation from the
soil, radon and from some construction materials is also not measured by this indicator.
Disclaimer 2 – for the indicators 'abiotic depletion potential for non-fossil resources', 'abiotic depletion potential for fossil resources',
'water (user) deprivation potential, deprivation-weighted water consumption', 'potential comparative toxic unit for ecosystems', 'potential
comparative toxic unit for humans – cancerogenic', 'Potential comparative toxic unit for humans - not cancerogenic', 'potential soil
quality index'. The results of this environmental impact indicator shall be used with care as the uncertainties on these results are high
as there is limited experience with the indicator. This EPD was created using a software tool.
References
AS 1012.9:2014
Methods of testing concrete - Method 9: Determination of the Further References
compressive strength of concrete specimens
IBU General Instructions
AS 1012.18-1996 (R-2014) General Instructions for the EPD programme of Institut Bauen
Methods of testing concrete - Method 18: Determination of und Umwelt e.V., Version 2.1, Berlin: Institut Bauen und Umwelt
setting time of fresh concrete, mortar and grout by penetration e.V., 2022, www.ibu-epd.com
resistance
LCA Calculator
AS 1478.1-2000 LCA Calculator software (version 6), by Sphera Solutions
Chemical admixtures for concrete, mortar and grout - Part 1: GmbH, Leinfelden-Echterdingen, 2024
Admixtures for concrete
LCA for Expert
Candidate List of SVHC Life cycle assessment software (version 10), by Sphera
Candidate List of Substances of Very High Concern for Solutions GmbH, Leinfelden-Echterdingen, 2022,
Authorisation, European Chemicals Agency (ECHA), 2024, https://sphera.com/life-cycle-assessment-lca-software/
https://echa.europa.eu/candidate-list-table
Managed LCA Content
EN 15804:2012+A2:2019+AC:2021 Life Cycle Assessment databases, Sphera Solutions GmbH,
Sustainability of construction works — Environmental Product Leinfelden-Echterdingen, 2022, https://sphera.com/life-cycle-
Declarations — Core rules for the product category of assessment-lca-database/
construction products
PCR Part A
ISO 14025:2011 PCR - Part A: Calculation rules for the Life Cycle Assessment
Environmental labels and declarations — Type III and Requirements on the Background Report, version 1.4,
environmental declarations — Principles and procedures Institut Bauen und Umwelt e.V., 04-2024
Model WHS Regulations PCR Part B
Schedule 10 Prohibited carcinogens, restricted carcinogens PCR – Part B: Requirements on the EPD for Concrete
and restricted hazardous chemicals, Australian Model Work admixtures, Institut Bauen und Umwelt e.V., 04-2023
Health and Safety Regulations, 08-2023
5 Environmental Product Declaration - Sika Australia Pty Ltd - Sika® Set Accelerator
Publisher
Institut Bauen und Umwelt e.V. +49 (0)30 3087748- 0
Hegelplatz 1 info@ibu-epd.com
10117 Berlin www.ibu-epd.com
Germany
Programme holder
Institut Bauen und Umwelt e.V. +49 (0)30 3087748- 0
Hegelplatz 1 info@ibu-epd.com
10117 Berlin www.ibu-epd.com
Germany
Author of the Life Cycle Assessment
Sphera Solutions GmbH +49 (0)711 341817-0
Hauptstraße 111- 113 info@sphera.com
70771 Leinfelden-Echterdingen www.sphera.com
Germany
Owner of the Declaration
Sika Australia Pty Ltd +61 2 9725 1145
Elizabeth Street 55 sustainability@au.sika.com
2164 Wetherill Park, NSW aus.sika.com
Australia
6 Environmental Product Declaration - Sika Australia Pty Ltd - Sika® Set Accelerator
