ENVIRONMENTAL PRODUCT DECLARATION
as per ISO 14025 and EN 15804+A2
Owner of the Declaration dormakaba International Holding GmbH
Publisher Institut Bauen und Umwelt e.V. (IBU)
Programme holder Institut Bauen und Umwelt e.V. (IBU)
Declaration number EPD-DOR-20210304-CBA8-EN
Issue date 04.05.2022
Valid to 03.05.2027
BEST 1C Series
dormakaba
www.ibu-epd.com | https://epd-online.com
General Information
dormakaba BEST 1C Series
Programme holder Owner of the declaration
IBU – Institut Bauen und Umwelt e.V. dormakaba International Holding GmbH
Hegelplatz 1 DORMA Platz 1
10117 Berlin 58256 Ennepetal
Germany Germany
Declaration number Declared product / declared unit
EPD-DOR-20210304-CBA8-EN 1 core (1 piece) of the BEST 1C Series.
This declaration is based on the product category rules: Scope:
Building Hardware products, 01.08.2021 This Environmental Product Declaration refers to a specific core
(PCR checked and approved by the SVR) manufactured by dormakaba. The production site is located in Indianapolis
(USA).
Issue date The data represents the year 2020.
The owner of the declaration shall be liable for the underlying information
04.05.2022
and evidence; the IBU shall not be liable with respect to manufacturer
information, life cycle assessment data and evidences.
Valid to
The EPD was created according to the specifications of EN 15804+A2. In
03.05.2027 the following, the standard will be simplified as EN 15804.
Verification
The standard EN 15804 serves as the core PCR
Independent verification of the declaration and data according to ISO
14025:2011
internally X externally
Dipl.-Ing. Hans Peters
(Chairman of Institut Bauen und Umwelt e.V.)
Florian Pronold Dr.-Ing. Wolfram Trinius,
(Managing Director Institut Bauen und Umwelt e.V.) (Independent verifier)
1 Environmental Product Declaration - dormakaba - BEST 1C Series
Product
Performance data of the product with respect to its
Product description/Product definition characteristics in accordance with the relevant technical
BEST Cores draw on the legacy of quality and expertise that provision which can be applied are mentioned above.
keep our products on the forefront of the industry. Brass alloy
construction result in reliable performance over time. BEST Base materials/Ancillary materials
Cores allow for easier rekeying by allow a user to remove the Name Value Unit
core from the lock without the need to remove the lever. For the
Brass 93 %
use and application of the product the respective national
Steel 3 %
provisions at the place of use apply. The standards which can
Paper 2 %
be applied are the following:
Others >2 %
• ANSI/BHMA 156.5
• BAA/TAA The product/s include/s partial articles which contain
• UL listed substances listed in the Candidate List of REACH Regulation
1907/2006/EC (date: 17.01.2022) exceeding 0.1 percentage by
Application mass: yes
BEST Cores are designed for commercial and institutional
• Lead (Pb): 7439-92-1 (CAS-No.) is included in some of
applications, where seamless removal of the core from its
the alloys used. The concentration of lead in each
hardware is needed.
individual alloy does not exceed 4.0% (by mass).
Technical Data
The Candidate List can be found on the ECHA website
The cores have following technical properties:
address: https://echa.europa.eu/de/home.
Reference service life
The reference service life of the BEST 1C Series cores depend
on the traffic pattern and degree of usage of the core. The
BEST 1C Series is certified to BHMA/ANSI Grade 1, meaning
they are designed to whithstand a minimum of 40,000 uses.
LCA: Calculation rules
Declared Unit System boundary
The declared unit is 1 piece of the product: BEST 1C Series. The type of EPD is: cradle to gate with options, modules C1–
Name Value Unit C4, and module D (A1–A3 + C + D and additional modules: A4
+ A5)
Declared unit 1 piece/product
Mass of declared Product 0.0449 kg
Production - Module A1-A3
2 Environmental Product Declaration - dormakaba - BEST 1C Series
The product stage includes: — C3, waste processing for reuse, recovery and/or recycling;
— A1, raw material extraction, processing and mechanical — C4, disposal; including provision and all transport, provision
treatments, processing of secondary material input (e.g. of all materials, products and related energy and water use.
recycling processes), - Module D (Benefits and loads beyond the system boundary)
— A2, transport to the manufacturer, includes:
— A3, manufacturing and assembly including provision of all — D, recycling potentials, expressed as net impacts and
materials, products and energy, as well as waste processing up benefits.
to the end-of waste state.
Construction stage - Modules A4-A5 Geographic Representativeness
The construction process stage includes: Land or region, in which the declared product system is
— A4, transport to the building site; manufactured, used or handled at the end of the product´s
— A5, installation into the building; including provision of all lifespan: United States
materials, products and energy, as well as waste processing up
to the end-of waste state or disposal of final residues during the
Comparability
construction process stage.
Basically, a comparison or an evaluation of EPD data is only
possible if all the data sets to be compared were created
End-of-life stage– Modules C1-C4 and D
according to EN 15804 and the building context, respectively
The end-of-life stage includes:
the product-specific characteristics of performance, are taken
— C1, de-construction, demolition:
into account.
— C2, transport to waste processing;
LCA: Scenarios and additional technical information
Installation into the building (A5)
Characteristic product properties of biogenic carbon
Name Value Unit
Information on describing the biogenic Carbon Content at
Output substances following waste treatment on
factory gate 0.0011 kg
site (packaging)
Name ValueUnit
Biogenic carbon content in accompanying kg End of life (C1-C4)
-
packaging C C1: The product dismantling from the building is done manually
without environmental burden.
C2: Transport to waste treatment at end of life is 50km.
Name Value Unit
Transport to the building site (A4)
Collected separately waste type 0.0438 kg
Name Value Unit
Recycling 0.0438 kg
Litres of fuel per 1 kg (truck) 0.00276l/100km
Transport distance truck 1500 km Reuse, recovery and/or recycling potentials (D), relevant
Capacity utilisation (including empty runs) scenario information
55 %
average Name Value Unit
Transport distance (ship) 10000 km
Collection rate is 100%.
3 Environmental Product Declaration - dormakaba - BEST 1C Series
LCA: Results
DESCRIPTION OF THE SYSTEM BOUNDARY (X = INCLUDED IN LCA; MND = MODULE OR INDICATOR NOT DECLARED; MNR
= MODULE NOT RELEVANT)
Benefits and
Construction loads beyond
Product stage Use stage End of life stage
process stage the system
boundaries
la ire ta m w a Ry lp p u s tro p s n a rT g n iru tc a fu n a M e h t m o rf tro p s n a rTe tis e h t o t e ta g y lb m e s s A e s U e c n a n e tn ia M ria p e R tn e m e c a lp e R tn e m h s ib ru fe R y g re n e la n o ita re p Oe s u re ta w la n o ita re p Oe s u n o itc u rts n o c -e Dn o itilo m e d tro p s n a rT g n is s e c o rp e ts a W la s o p s iD -e s u e R-y re v o c e R-g n ilc y c e Rla itn e to p
A1 A2 A3 A4 A5 B1 B2 B3 B4 B5 B6 B7 C1 C2 C3 C4 D
X X X X X MND MND MNR MNR MNR MND MND X X X X X
RESULTS OF THE LCA - ENVIRONMENTAL IMPACT according to EN 15804+A2: 1 core
Parameter Unit A1-A3 A4 A5 C1 C2 C3 C4 D
GWP-total kg CO 2 eq 3.1E-01 7E-03 2E-03 0 1.92E-04 0 0 2E-03
GWP-fossil kg CO 2 eq 3E-01 7E-03 3.91E-05 0 1.83E-04 0 0 2E-03
GWP-biogenic kg CO 2 eq 9.05E-03 2.62E-04 2E-03 0 8.46E-06 0 0 -3.56E-06
GWP-luluc kg CO 2 eq 1.59E-04 1.64E-07 2.57E-08 0 4.36E-09 0 0 3.03E-06
ODP kg CFC11 eq 1.35E-14 7.33E-19 2.81E-19 0 1.93E-20 0 0 6.35E-18
AP mol H+ eq 9.26E-04 5.97E-05 4.37E-07 0 1.83E-07 0 0 4.24E-05
EP-freshwater kg P eq 2.52E-07 1.54E-09 5.5E-11 0 3.92E-11 0 0 8.54E-09
EP-marine kg N eq 1.28E-04 1.61E-05 1.58E-07 0 5.83E-08 0 0 2.41E-06
EP-terrestrial mol N eq 1.38E-03 1.76E-04 1.97E-06 0 6.48E-07 0 0 2.62E-05
kg NMVOC
POCP 3.83E-04 4.5E-05 4.18E-07 0 1.65E-07 0 0 8.55E-06
eq
ADPE kg Sb eq 2.04E-05 2.07E-10 4.44E-12 0 5.49E-12 0 0 4.43E-06
ADPF MJ 4.74E+00 9.8E-02 4.92E-04 0 3E-03 0 0 2.4E-02
m3 world eq
WDP 6.9E-02 1.37E-05 1.93E-04 0 3.59E-07 0 0 1E-03
deprived
GWP = Global warming potential; ODP = Depletion potential of the stratospheric ozone layer; AP = Acidification potential of land and water; EP =
Eutrophication potential; POCP = Formation potential of tropospheric ozone photochemical oxidants; ADPE = Abiotic depletion potential for non-fossil
resources; ADPF = Abiotic depletion potential for fossil resources; WDP = Water (user) deprivation potential)
RESULTS OF THE LCA - INDICATORS TO DESCRIBE RESOURCE USE according to EN 15804+A2: 1 core
Parameter Unit A1-A3 A4 A5 C1 C2 C3 C4 D
PERE MJ 8.52E-01 3.1E-04 1.3E-02 0 8.19E-06 0 0 7E-03
PERM MJ 1.3E-02 0 -1.3E-02 0 0 0 0 0
PERT MJ 8.65E-01 3.1E-04 8.95E-05 0 8.19E-06 0 0 7E-03
PENRE MJ 4.74E+00 9.8E-02 4.93E-04 0 3E-03 0 0 2.5E-02
PENRM MJ 0 0 0 0 0 0 0 0
PENRT MJ 4.74E+00 9.8E-02 4.93E-04 0 3E-03 0 0 2.5E-02
SM kg 4.5E-02 0 0 0 0 0 0 0
RSF MJ 0 0 0 0 0 0 0 0
NRSF MJ 0 0 0 0 0 0 0 0
FW m3 2.44E-03 5.58E-07 4.55E-06 0 1.47E-08 0 0 6.98E-06
PERE = Use of renewable primary energy excluding renewable primary energy resources used as raw materials; PERM = Use of renewable primary
energy resources used as raw materials; PERT = Total use of renewable primary energy resources; PENRE = Use of non-renewable primary energy
excluding non-renewable primary energy resources used as raw materials; PENRM = Use of non-renewable primary energy resources used as raw
materials; PENRT = Total use of non-renewable primary energy resources; SM = Use of secondary material; RSF = Use of renewable secondary fuels;
NRSF = Use of non-renewable secondary fuels; FW = Use of net fresh water
RESULTS OF THE LCA – WASTE CATEGORIES AND OUTPUT FLOWS according to EN 15804+A2:
1 core
Parameter Unit A1-A3 A4 A5 C1 C2 C3 C4 D
HWD kg 4.06E-09 9.5E-12 7.26E-13 0 2.52E-13 0 0 2.8E-10
NHWD kg 1.5E-02 9.99E-06 4.89E-05 0 2.66E-07 0 0 1.01E-04
RWD kg 4.14E-04 1.06E-07 2.59E-08 0 2.79E-09 0 0 1.1E-06
CRU kg 0 0 0 0 0 0 0 0
MFR kg 0 0 0 0 0 4.4E-02 0 0
MER kg 0 0 0 0 0 0 0 0
EEE MJ 1.7E-02 0 2E-03 0 0 0 0 0
EET MJ 3.1E-02 0 4E-03 0 0 0 0 0
HWD = Hazardous waste disposed; NHWD = Non-hazardous waste disposed; RWD = Radioactive waste disposed; CRU = Components for re-use;
MFR = Materials for recycling; MER = Materials for energy recovery; EEE = Exported electrical energy; EET = Exported thermal energy
4 Environmental Product Declaration - dormakaba - BEST 1C Series
RESULTS OF THE LCA – additional impact categories according to EN 15804+A2-optional:
1 core
Parameter Unit A1-A3 A4 A5 C1 C2 C3 C4 D
Disease
PM 7.66E-09 9.54E-10 2.42E-12 0 9.63E-13 0 0 3.09E-10
incidence
IR kBq U235 eq 3.8E-02 1.51E-05 4.01E-06 0 3.99E-07 0 0 -8.56E-05
ETP-fw CTUe 1.78E+00 6.9E-02 2.34E-04 0 2E-03 0 0 4.1E-02
HTP-c CTUh 1.9E-10 1.3E-12 1.24E-14 0 3.46E-14 0 0 7.09E-13
HTP-nc CTUh 2.95E-09 5.68E-11 5.36E-13 0 1.48E-12 0 0 2.17E-10
SQP SQP 9E-01 2.53E-04 1.31E-04 0 6.67E-06 0 0 2.3E-02
PM = Potential incidence of disease due to PM emissions; IR = Potential Human exposure efficiency relative to U235; ETP-fw = Potential comparative
Toxic Unit for ecosystems; HTP-c = Potential comparative Toxic Unit for humans (cancerogenic); HTP-nc = Potential comparative Toxic Unit for humans
(not cancerogenic); SQP = Potential soil quality index
Disclaimer 1 – for the indicator “Potential Human exposure efficiency relative to U235”. This impact category deals mainly with the
eventual impact of low-dose ionizing radiation on human health of the nuclear fuel cycle. It does not consider effects due to possible
nuclear accidents, occupational exposure or radioactive waste disposal in underground facilities. Potential ionizing radiation from the
soil, radon and from some construction materials is also not measured by this indicator.
Disclaimer 2 – for the indicators “abiotic depletion potential for non-fossil resources”, “abiotic depletion potential for fossil resources”,
“water (user) deprivation potential, deprivation-weighted water consumption”, “potential comparative toxic unit for ecosystems”,
“potential comparative toxic unit for humans – cancerogenic”, “Potential comparative toxic unit for humans - not cancerogenic”,
“potential soil quality index”. The results of this environmental impact indicator shall be used with care as the uncertainties on these
results are high as there is limited experience with the indicator.
References
Standards Further References
EN 15804 Buy American Act
EN 15804:2012+A1 2013, Sustainability of construction works https:/www.goa.gov/products/105519
— Environmental Product Declarations — Core rules for the
product category of construction products. Trade Agreements Act
https://vsc.gsa.gov/administration/compDetails.cfm.
EN 15804
EN 15804:2012+A2:2019+AC:2021, Sustainability of GaBi ts software
construction works — Environmental Product Declarations — Sphera Solutions GmbH
Core rules for the product category of construction products. Gabi Software System and Database for Life Cycle Engineering
1992-2020
ISO 14025 Version 10.0.0.71
EN ISO 14025:2011, Environmental labels and declarations — University of Stuttgart
Type III environmental declarations — Principles and Leinfelden-Echterdingen
procedures.
GaBi ts documentation
Further References GaBi life cycle inventory data documentation (https://www.gabi-
software.com/support/gabi/gabidatabase-
IBU 2021 2020-lci-documentation/).
Institut Bauen und Umwelt e.V.: General Instructions for the
EPD programme of Institut Bauen und Umwelt e.V., Version LCA-tool dormakaba
2.0, Berlin: Institut Bauen und Umwelt e.V., 2021 LCA-tool, IBU-DOR-202104-LT1-EN.
www.ibu-epd.com Developed by Sphera Solutions GmbH
ANSI/BHMA A156.5 PCR Part A
ANSI/BHMA A156.4 - 2014, Cylinders and Input Devices for PCR – Part A: Calculation Rules for the Life Cycle Assessment
Locks. and Requirements on the Project Re-port
according to EN 15804+A2:2019, Version 1.0, 2020, Institut
EN 15804:2019+A2 Bauen und Umwelt e.V., www.ibu-epd.com.
EN 15804:2019+A2 (in press), Sustainability of construction
works — Environmental Product Declarations — Core rules for PCR Part B
the product category of construction products. PCR – Part B: Requirements on the EPD for Building Hardware
product, version 1.2, Institut Bauen und
Registration, Evaluation, Authorisation and Restriction of Umwelt e.V., www.ibu-epd.com, 2017.
Chemicals (REACH)
Regulation (EC) No 1907/2006 of the European Parliament and Underwriters Laboratories
of the Council on the Registration, Evaluation, Authorisation https://www.ul.com/.
and Restriction of Chemicals (REACH).
5 Environmental Product Declaration - dormakaba - BEST 1C Series
Publisher
Institut Bauen und Umwelt e.V. +49 (0)30 3087748- 0
Hegelplatz 1 info@ibu-epd.com
10117 Berlin www.ibu-epd.com
Germany
Programme holder
Institut Bauen und Umwelt e.V. +49 (0)30 3087748- 0
Hegelplatz 1 info@ibu-epd.com
10117 Berlin www.ibu-epd.com
Germany
Author of the Life Cycle Assessment
Sphera Solutions GmbH +49 711 341817-0
Hauptstraße 111- 113 info@sphera.com
70771 Leinfelden-Echterdingen www.sphera.com
Germany
Owner of the Declaration
dormakaba International Holding GmbH +49 2333 793-0
DORMA Platz 1 info.de@dormakaba.com
58256 Ennepetal www.dormakaba.com
Germany
6 Environmental Product Declaration - dormakaba - BEST 1C Series
