Environmental Product Declaration (EPD)
According to ISO 14025 and EN 15804
ACEFormer™
Registration number: EPD-Kiwa-EE-158053-EN
Issue date: 22-12-2023
Valid until: 22-12-2028
Declaration owner: Gold-Joint Industry Co., Ltd.
Publisher: Kiwa-Ecobility Experts
Program operator: Kiwa-Ecobility Experts
Status: verified
ACEFormer™ | ReTHiNK-58053 1 / 24
Environmental Product Declaration
1 General information
E-mail: marketing@geoace.com
1.1 PRODUCT Website: www.geoace.com
Production location: Gold-Joint Industry Co., Ltd.
ACEFormer™
Address production location: No.33, Jing 3 Rd. Wuqi Dist., 43541 Taichung City
1.2 REGISTRATION NUMBER
1.6 VERIFICATION OF THE DECLARATION
EPD-Kiwa-EE-158053-EN
The independent verification is in accordance with the ISO 14025:2011. The LCA is in
1.3 VALIDITY compliance with ISO 14040:2006 and ISO 14044:2006. The EN 15804:2012+A2:2019 serves as
the core PCR.
Issue date: 22-12-2023
Internal ✓ External
Valid until: 22-12-2028
1.4 PROGRAM OPERATOR
Kiwa-Ecobility Experts
Voltastraße 5
13355 Berlin
DE
Elisabeth Amat Guasch, Greenize
1.7 STATEMENTS
Prof. Dr. Frank Heimbecher
The owner of this EPD shall be liable for the underlying information and evidence. The
(Chairman of the independent expert
programme operator Kiwa-Ecobility Experts shall not be liable with respect to
committee - Kiwa-Ecobility Experts)
manufacturer data, life cycle assessment data and evidence.
Frank Huppertz 1.8 PRODUCT CATEGORY RULES
(Head of Kiwa-Ecobility Experts)
Kiwa-Ecobility Experts (Kiwa-EE) – General Product Category Rules (2022-02-14)
Kiwa-Ecobility Experts (Kiwa-EE) – Specific Product Category Rules: Geosynthetic products
1.5 OWNER OF THE DECLARATION
(2023-07-21)
Manufacturer: Gold-Joint Industry Co., Ltd.
Address: No.33, Jing 3 Rd. Wuqi Dist., 43541 Taichung City, Taiwan (R.O.C.)
ACEFormer™ | ReTHiNK-58053 2 / 24
Environmental Product Declaration
1 General information
1.9 COMPARABILITY 1.10 CALCULATION BASIS
In principle, a comparison or assessment of the environmental impacts of different LCA method R<THiNK: Ecobility Experts | EN15804+A2
products is only possible if they have been prepared in accordance with EN 15804. For the
evaluation of the comparability, the following aspects have to be considered in particular: LCA software*: Simapro 9.1
PCR used, functional or declared unit, geographical reference, the definition of the system Characterization method: EN 15804 +A2 Method v1.0
boundary, declared modules, data selection (primary or secondary data, background
database, data quality), scenarios used for use and disposal phases, and the life cycle LCA database profiles: EcoInvent version 3.6
inventory (data collection, calculation methods, allocations, validity period). PCRs and Version database: v3.15 (2023-07-12)
general program instructions of different EPDs programs may differ. Comparability needs
to be evaluated. For further guidance, see EN 15804+A2 (5.3 Comparability of EPD for
*Used for calculating the characterized results of the Environmental profiles within
construction products) and ISO 14025 (6.7.2 Requirements for comparability).
R<THiNK.
1.11 LCA BACKGROUND REPORT
This EPD is generated on the basis of the LCA background report 'ACEFormer™' with the
calculation identifier ReTHiNK-58053.
ACEFormer™ | ReTHiNK-58053 3 / 24
Environmental Product Declaration
2 Product
2.1 PRODUCT DESCRIPTION Further versatility is seen in applications like slope stabilization and constructing
revetments. Their adaptability suits them for projects with diverse demands.
ACEFormer™ geotextile mattress is a dual-layer structured fabric, capable of being filled
2.3 REFERENCE SERVICE LIFE
with high-strength fine aggregate concrete or cement mortar to function as a protective
lining system. Its merits include adaptability to various terrains, simple and rapid
construction, excellent integrity once installed, and strong resistance to erosion. The RSL PRODUCT
geotextile mattress can be installed on land, underwater, or steep slopes for applications According to application standards (EN 13249-13257, EN 13265, and EN 15381) and the
such as riverbank revetment, channel protection, underwater lining, and pipeline Taiwanese Design Code, the typical Reference Serviceis Life (RSL) of ACEFormer™
protection. Customized to meet local conditions, the geotextile mattress offers superb approximately 50 years.
flexibility and presents significant advantages over traditional concrete solutions due to its
ability to conform excellently to diverse application environments. USED RSL (YR) IN THIS LCA CALCULATION:
The following products are covered in this EPD: V-Type, F-Type, L-Type, T-Type, U-Type and 50
P-Type.
2.4 TECHNICAL DATA
See above (2.1).
2.5 SUBSTANCES OF VERY HIGH CONCERN
The product contains less than 0.1% of substances included in the “Candidate list of
substances of very high concern for authorisation” (SVHC).
2.6 DESCRIPTION PRODUCTION PROCESS
PET yarn and PP yarn are the raw materials used in the production of ACEFormer™. Prior
to production, the original yarn must be twisted into processed yarn, an operation carried
out by external partners. Once the twisting process is complete, the yarn is trucked back to
the Gold-Joint factory for further processing.
Post the warping process, the processed yarn can be fed into the production line for
weaving geotextile mattresses. Weaving is a fabric production method where two distinct
sets of yarn interlace at right angles, forming a longitudinal warp direction (machine
direction) and a transversal weft direction (cross-machine direction). Through specific
2.2 APPLICATION (INTENDED USE OF THE PRODUCT)
design of the textile structure, both single-layer and double-layer fabrics can be produced,
with their sizes adjustable based on application requirements.
ACEFormer™ geotextile mattresses are specialized for hydraulic and erosion control uses.
Notably, they're employed in riverbank stabilization projects, where they are studied for After weaving, the fabric is rolled onto beams and sent to the internal processing
their ability to prevent soil erosion, especially with the rise in flood events. Their utility in department for sewing operations. Since geotextile mattresses are custom-made
preserving both natural habitats and human-made structures near coastlines is under products, the processing is done according to the specifications, forms, sizes, and
scrutiny. ACEFormer™ also find use in scour prevention. They're applied at the bases of accessories required by the order. Before the sewing process begins, the fabric is inspected
structures like piers and embankments, where water-induced erosion could threaten for defects. The fabric is then cut and
stability. Engineers are assessing their short and long-term performance in these contexts.
ACEFormer™ | ReTHiNK-58053 4 / 24
Environmental Product Declaration
2 Product
sewn according ortode r requirements, and necessary parts (e .g., handler loops, zippers)
are sewn and affithxee d prtoo duct. -Placement of ACEFormer™
Upon completion, quality control personnel measure the fin al produ-ct'Ancsho rdiamgeen spirooncess sand
count the number of accessories using a production checklist . After careful inspection of
-Filling of the panels with flowable concrete/mortar
the sewing areas, the product is folded and packaged.
2.7 CONSTRUCTION DESCRIPTION
The construction process of ACEFormer™ can be divided into the following parts:
-Preparation of the site
ACEFormer™ | ReTHiNK-58053 5 / 24
Environmental Product Declaration
3 Calculation rules
3.1 DECLARED UNIT Module B2 = Maintenance Module C4 = Disposal
Module D = Benefits and loads beyond the
One square meter ACEFormer™ Module B3 = Repair
product system boundaries
m² of ACEFormer™. The following products are covered in this EPD: V-Type, F-Type, L-Type,
Module B4 = Replacement
T-Type, U-Type and P-Type.
reference_unit: square meter (m2)
3.4 REPRESENTATIVENESS
3.2 CONVERSION FACTORS
The input data are representative for ACEFormer™, a product of Gold-Joint Industry Co.,
Ltd.. The data are representative for Asia.
Description Value Unit
reference_unit 1 m2
3.5 CUT-OFF CRITERIA
weight_per_reference_unit 1.417 kg
Product Stage (A1-A3)
Conversion factor to 1 kg 0.705862 m2
All input flows (e.g. raw materials, transportation, energy use, packaging, etc.) and output
3.3 SCOPE OF DECLARATION AND SYSTEM BOUNDARIES flows (e.g. production waste) are considered in this LCA. The total neglected input flows do
therefore not exceed the limit of 5% of energy use and mass.
This is a Cradle to gate with options, modules C1-C4 and module D LCA. The life cycle
stages included are as shown below: Construction process stage (A4-A5)
(X = module included, ND = module not declared)
All input flows (e.g. transportation to the construction site, additional raw material use for
A1 A2 A3 A4 A5 B1 B2 B3 B4 B5 B6 B7 C1 C2 C3 C4 D
construction, installation energy (use)of energy use for assembly , etc.) and output flows
X X X X X ND ND ND ND ND ND ND X X X X X (e.g. construction waste, packaging waste, etc.) are considered in this LCA. The total
neglected input flows do therefore not exceed the limit of 5% of energy use and mass.
The modules of the EN15804 contain the following:
End of life stage (C1-C4)
Module A1 = Raw material supply Module B5 = Refurbishment
Module A2 = Transport Module B6 = Operational energy use All input flows (e.g. energy use for demolition or disassembly, transport to waste
processing, etc.) and output flows (e.g. end-of-life waste processing of the product, etc.) are
Module A3 = Manufacturing Module B7 = Operational water use
considered in this LCA. The total neglected input flows do therefore not exceed the limit of
Module A4 = Transport Module C1 = De-construction / Demolition 5% of energy use and mass.
Module A5 = Construction -
Module C2 = Transport
Installation process Benefits and Loads beyond the system boundary (Module D)
Module B1 = Use Module C3 = Waste Processing
ACEFormer™ | ReTHiNK-58053 6 / 24
Environmental Product Declaration
3 Calculation rules
All benefits and loads beyond the system boundary resulting from reusable products, The inputs PET raw yarn, PP raw yarn and PP chips also did not have a linear dependence
recyclable materials and/or useful energy carriers leaving the product system are on the specific mass. As they are the main inputs present in the product, the linear
considered in this LCA. dependence on the specific mass of the sum of these 3 inputs was calculated instead of
considering the inputs separately.
3.6 ALLOCATION The stirring materials (colour masterbatch, anti-UV masterbatch, thermoplastic elastomer)
and auxiliary materials were scaled to the amount of PP chips. This is because these
Allocation is based on physical characteristics (mass). The production data was calculated materials are only involved in the mixing process of the self-extruded material and not in
according to the annual quantity by mass. The raw materials and energy were calculated the outsourced yarn production.
according to this allocation key.
The linear dependence of energy consumption on specific mass has been calculated by
taking into account the sum of production energy and yarn twisting energy (which is
3.7 DATA COLLECTION & REFERENCE TIME PERIOD outsourced).
For C1 the method and amount of the generic data set 'Polyester weefsel' from chapter
All process-specific data was collected for the operating year 2021.
22.46 Grondwapening en grondscheiding of the DuboCalc programme (database version
NMD 1.8 - 5.01.14052018) was used. In this generic data set, 0.0013h work per m² of
3.8 ESTIMATES AND ASSUMPTIONS geotextile was assumed.
Almost all the datasets selected for the LCA refer to the RoW as the geographical
3.9 DATA QUALITY
reference, as there were no specific environmental profiles available.
Gold-Joint delivers its product to different countries, so the calculation of transport to All process-specific data was collected for the 2021 operating year and is therefore up-to-
construction site (A4) was done by taking the average distance, weighted by the date. The data is based on the annual average. In order to ensure comparability of the
proportion of product shipped to each country. For module A4, a data set for a non- results, only consistent background data of the Ecoinvent database V3.6 was used in the
specific truck and a transoceanic ship was used. LCA (e.g., records on energy, transportation, and supplies), which refers to reference year
2019. The database is regularly reviewed and thus complies with the requirements of EN
A scaling method was used to calculate the LCA results for the different ACEFormer™ 15804 (background data not older than 10 years). All consistent datasets contained in the
products. The scaling was done on the basis of mass per square meter. As a result of Ecoinvent database are documented and can be viewed in the online Ecoinvent
scaling there are results for both the fixed and the scalable part of the scaling function. documentation. The primary data were provided by Gold-Joint. The life cycle was modelled
The fixed part means that this number is the same for each product in the product group with the R<THiNK EPD App.
and the scalable part is the part that depends on the mass per unit area of the product. In
order to calculate the correct number of each environmental impact category for each of
the products in the product group, the following calculation should be done: 3.10 GUARANTEES OF ORIGIN
[number fixed part]+([specific mass]*[number scalable part]) In this EPD, the local based approach was considered for the LCA, therefore no guaranties
of origin (GO) are needed.
ACEFormer™ | ReTHiNK-58053 7 / 24
Environmental Product Declaration
3 Calculation rules
3.12 SCALING
Parameter Value
Scaling type Linear
Description dimension Specific mass
Dimension 0.000
Scalable dimension 1.000
Unit dimension kg/m²
ACEFormer™ | ReTHiNK-58053 8 / 24
Environmental Product Declaration
4 Scenarios and additional technical information
4.1 TRANSPORT TO CONSTRUCTION SITE (A4)
For the transport from production place to assembly/user, the following scenario is
assumed for module A4 of this EPD.
Value and unit
Vehicle type used for transport Transoceanic ship / Lorry unspecified
Fuel type and consumption of vehicle
Distance 2274 km
Capacity utilisation (including empty returns)
Bulk density of transported products
Volume capacity utilisation factor
4.2 ASSEMBLY (A5)
The following information describes the scenarios for flows entering the system and flows
leaving the system at module A5.
FLOWS ENTERING THE SYSTEM
There are no significant environment impacts as a result of materials or energy used in the
construction stage (A5).
FLOWS LEAVING THE SYSTEM
The following output flows leaving the system at module A5 are assumed.
Description Value Unit
Output materials as result of loss during construction 5 %
Output materials as result of waste processing of materials used for installation/assembly at the building site 0.000 kg
Output materials as result of waste processing of used packaging 0.012 kg
4.3 DE-CONSTRUCTION, DEMOLITION (C1)
The following information describes the scenario for demolition at end of life.
Description Amount Unit
Hydraulic excavator (average) [NMD] 0.001 hr
ACEFormer™ | ReTHiNK-58053 9 / 24
Environmental Product Declaration
4 Scenarios and additional technical information
4.4 TRANSPORT END-OF-LIFE (C2)
The following distances and transport conveyance are assumed for transportation during
end of life for the different types of waste processing.
Waste Scenario Transport conveyance Not removed (stays in Landfill Incineration Recycling Re-use
work) [km] [km] [km] [km] [km]
PE/PP soil reinforcement (geotextile and Lorry (Truck), unspecified (default) | market
0 100 150 50 0
geogrid 54) group for (GLO)
finishes (adhered to wood, plastic, metal) Lorry (Truck), unspecified (default) | market
0 100 150 50 0
(NMD ID 2) group for (GLO)
The transport conveyance(s) used in the scenario(s) for transport during end of life has the
following characteristics.
Value and unit
Vehicle type used for transport Lorry (Truck), unspecified (default) | market group for (GLO)
Fuel type and consumption of vehicle not available
Capacity utilisation (including empty returns) 50 % (loaded up and return empty)
Bulk density of transported products inapplicable
Volume capacity utilisation factor 1
4.5 END OF LIFE (C3, C4)
The scenario(s) assumed for end of life of the product are given in the following tables.
First the assumed percentages per type of waste processing are displayed, followed by the
assumed amounts.
Waste Scenario Region Not removed (stays in work) [%] Landfill [%] Incineration [%] Recycling [%] Re-use [%]
PE/PP soil reinforcement (geotextile and geogrid 54) NL 25 0 70 5 0
finishes (adhered to wood, plastic, metal) (NMD ID 2) NL 0 0 100 0 0
ACEFormer™ | ReTHiNK-58053 10 / 24
Environmental Product Declaration
4 Scenarios and additional technical information
Waste Scenario Not removed (stays in work) [kg] Landfill [kg] Incineration [kg] Recycling [kg] Re-use [kg]
PE/PP soil reinforcement (geotextile and geogrid 54) 0.447 0.000 1.251 0.089 0.000
Total 0.447 0.000 1.251 0.089 0.000
4.6 BENEFITS AND LOADS BEYOND THE SYSTEM BOUNDARY (D)
The presented Benefits and loads beyond the system boundary in this EPD are based on
the following calculated Net output flows in kilograms and Energy recovery displayed in
MJ Lower Heating Value.
Waste Scenario Net output flow [kg] Energy recovery [MJ]
PE/PP soil reinforcement (geotextile and geogrid 54) 0.071 27.664
finishes (adhered to wood, plastic, metal) (NMD ID 2) 0.000 0.000
Total 0.071 27.664
ACEFormer™ | ReTHiNK-58053 11 / 24
Environmental Product Declaration
5 Results
For the impact assessment, the characterization factors of the LCIA method EN 15804 +A2
Method v1.0 are used. Long-term emissions (>100 years) are not considered in the impact
assessment. The results of the impact assessment are only relative statements that do not
make any statements about end-points of the impact categories, exceedance of threshold
values, safety margins or risks. The following tables show the results of the indicators of the
impact assessment, of the use of resources as well as of waste and other output flows.
ACEFormer™ | ReTHiNK-58053 12 / 24
Environmental Product Declaration
5 Results
5.1 ENVIRONMENTAL IMPACT INDICATORS PER SQUARE METER (FIXED PART)
CORE ENVIRONMENTAL IMPACT INDICATORS EN15804+A2
Abbreviation Unit A1 A2 A3 A4 A5 C1 C2 C3 C4 D
AP mol H+ eqv. -4.40E-3 -2.22E-4 -4.63E-3 -2.84E-4 -4.83E-4 7.12E-4 -3.12E-5 -3.14E-4 -8.56E-6 3.98E-4
GWP-total kg CO2 eqv. -1.04E+0 -6.83E-3 -1.12E+0 -2.42E-2 -1.19E-1 6.81E-2 -5.38E-3 -6.96E-1 -1.37E-2 3.57E-1
GWP-b kg CO2 eqv. -2.44E-3 2.07E-6 4.62E-3 -1.50E-5 5.25E-3 1.89E-5 -2.48E-6 -1.01E-4 -1.06E-5 2.83E-4
GWP-f kg CO2 eqv. -1.03E+0 -6.83E-3 -1.12E+0 -2.42E-2 -1.24E-1 6.81E-2 -5.37E-3 -6.95E-1 -1.37E-2 3.57E-1
GWP-luluc kg CO2 eqv. -6.25E-4 -4.72E-6 -6.66E-5 -1.00E-5 -3.64E-5 5.37E-6 -1.97E-6 -5.65E-5 -4.85E-7 1.95E-5
EP-m kg N eqv. -8.22E-4 -5.46E-5 -6.12E-4 -7.04E-5 -7.98E-5 3.14E-4 -1.10E-5 -8.57E-5 -5.19E-6 1.02E-4
EP-fw kg P eqv. -2.37E-4 -2.80E-8 -4.47E-5 -2.85E-7 -1.41E-5 2.48E-7 -5.42E-8 -2.10E-6 -1.76E-8 9.85E-7
EP-T mol N eqv. -8.57E-3 -6.07E-4 -6.84E-3 -7.85E-4 -8.60E-4 3.45E-3 -1.21E-4 -9.55E-4 -3.15E-5 1.12E-3
kg CFC 11
ODP -3.61E-8 -1.37E-9 -4.99E-8 -5.15E-9 -5.18E-9 1.47E-8 -1.19E-9 -2.13E-8 -3.04E-10 4.24E-8
eqv.
kg NMVOC
POCP -3.25E-3 -1.57E-4 -2.03E-3 -2.15E-4 -2.88E-4 9.49E-4 -3.46E-5 -2.57E-4 -1.21E-5 4.11E-4
eqv.
ADP-f MJ -2.79E+1 -8.73E-2 -1.51E+1 -3.57E-1 -2.20E+0 9.37E-1 -8.10E-2 -5.42E-1 -2.32E-2 6.68E+0
ADP-mm kg Sb-eqv. -1.38E-5 -5.08E-8 -1.59E-6 -4.23E-7 -8.09E-7 1.04E-7 -1.36E-7 -8.92E-7 -1.05E-8 4.26E-7
m3 world
WDP -4.11E-1 -1.27E-4 -1.50E-1 -1.57E-3 -2.89E-2 1.26E-3 -2.90E-4 -3.55E-2 -9.95E-4 5.39E-2
eqv.
AP=Acidification (AP) | GWP-total=Global warming potential (GWP-total) | GWP-b=Global warming potential - Biogenic (GWP-b) | GWP-f=Global warming potential - Fossil (GWP-f) | GWP-
luluc=Global warming potential - Land use and land use change (GWP-luluc) | EP-m=Eutrophication marine (EP-m) | EP-fw=Eutrophication, freshwater (EP-fw) | EP-T=Eutrophication,
terrestrial (EP-T) | ODP=Ozone depletion (ODP) | POCP=Photochemical ozone formation - human health (POCP) | ADP-f=Resource use, fossils (ADP-f) | ADP-mm=Resource use, minerals and
metals (ADP-mm) | WDP=Water use (WDP)
ACEFormer™ | ReTHiNK-58053 13 / 24
Environmental Product Declaration
5 Results
ADDITIONAL ENVIRONMENTAL IMPACT INDICATORS EN15084+A2
Abbreviation Unit A1 A2 A3 A4 A5 C1 C2 C3 C4 D
ETP-fw CTUe -1.35E+1 -5.62E-2 -1.14E+1 -2.94E-1 -1.43E+0 5.65E-1 -7.23E-2 -8.74E+0 -2.47E-2 5.22E-1
disease
PM -3.65E-8 -2.10E-10 -1.16E-8 -1.71E-9 -2.55E-9 1.89E-8 -4.83E-10 -2.54E-9 -1.62E-10 1.87E-9
incidence
HTP-c CTUh -3.42E-10 -3.87E-12 -2.38E-10 -9.65E-12 -3.20E-11 1.97E-11 -2.34E-12 -1.33E-10 -6.48E-13 3.01E-11
HTP-nc CTUh -8.87E-9 -4.49E-11 -7.90E-9 -2.98E-10 -9.08E-10 4.85E-10 -7.91E-11 -2.76E-9 -1.61E-11 5.18E-10
IR kBq U235 eqv. -4.77E-2 -3.74E-4 -4.52E-2 -1.52E-3 -4.79E-3 4.02E-3 -3.40E-4 -2.22E-3 -9.10E-5 2.61E-3
SQP Pt -1.75E+0 -1.18E-2 -1.39E+0 -2.27E-1 -1.76E-1 1.20E-1 -7.03E-2 -2.00E-1 -5.49E-2 -3.67E-2
ETP-fw=Ecotoxicity, freshwater (ETP-fw) | PM=Particulate Matter (PM) | HTP-c=Human toxicity, cancer (HTP-c) | HTP-nc=Human toxicity, non-cancer (HTP-nc) | IR=Ionising radiation, human
health (IR) | SQP=Land use (SQP)
CLASSIFICATION OF DISCLAIMERS TO THE DECLARATION OF CORE AND ADDITIONAL ENVIRONMENTAL IMPACT INDICATORS
ILCD classification Indicator Disclaimer
Global warming potential (GWP) None
ILCD type / level 1 Depletion potential of the stratospheric ozone layer (ODP) None
Potential incidence of disease due to PM emissions (PM) None
AAcidification potential, Accumulated Exceedance (AP) None
Eutrophication potential, Fraction of nutrients reaching freshwater end compartment
None
(EP-freshwater)
Eutrophication potential, Fraction of nutrients reaching marine end compartment
ILCD type / level 2 None
(EP-marine)
Eutrophication potential, Accumulated Exceedance (EP-terrestrial) None
Formation potential of tropospheric ozone (POCP) None
Potential Human exposure efficiency relative to U235 (IRP) 1
Abiotic depletion potential for non-fossil resources (ADP-minerals&metals) 2
ILCD type / level 3
Abiotic depletion potential for fossil resources (ADP-fossil) 2
Water (user) deprivation potential, deprivation-weighted water consumption (WDP) 2
Potential Comparative Toxic Unit for ecosystems (ETP-fw) 2
ACEFormer™ | ReTHiNK-58053 14 / 24
Environmental Product Declaration
5 Results
ILCD classification Indicator Disclaimer
Potential Comparative Toxic Unit for humans (HTP-c) 2
Potential Comparative Toxic Unit for humans (HTP-nc) 2
Potential Soil quality index (SQP) 2
Disclaimer 1 – This impact category deals mainly with the eventual impact of low dose ionizing radiation on human health of the nuclear fuel cycle. It does not consider effects due to possible
nuclear accidents, occupational exposure nor due to radioactive waste disposal in underground facilities. Potential ionizing radiation from the soil, from radon and from some construction
materials is also not measured by this indicator.
Disclaimer 2 – The results of this environmental impact indicator shall be used with care as the uncertainties on these results are high or as there is limited experienced with the indicator.
5.2 ENVIRONMENTAL IMPACT INDICATORS PER SQUARE METER (SCALABLE PART)
CORE ENVIRONMENTAL IMPACT INDICATORS EN15804+A2
Abbreviation Unit A1 A2 A3 A4 A5 C1 C2 C3 C4 D
AP mol H+ eqv. 2.11E-2 1.02E-3 2.88E-2 1.41E-3 2.70E-3 0.00E+0 1.50E-4 1.51E-3 4.13E-5 -1.94E-3
GWP-total kg CO2 eqv. 4.95E+0 3.19E-2 6.94E+0 1.21E-1 7.80E-1 0.00E+0 2.59E-2 3.36E+0 6.63E-2 -1.74E+0
GWP-b kg CO2 eqv. 1.10E-2 -9.06E-6 -2.87E-2 7.46E-5 -8.54E-4 0.00E+0 1.20E-5 4.86E-4 5.10E-5 -1.38E-3
GWP-f kg CO2 eqv. 4.94E+0 3.19E-2 6.97E+0 1.20E-1 7.80E-1 0.00E+0 2.59E-2 3.36E+0 6.63E-2 -1.74E+0
GWP-luluc kg CO2 eqv. 2.92E-3 2.18E-5 5.14E-4 4.99E-5 1.90E-4 0.00E+0 9.50E-6 2.73E-4 2.34E-6 -1.02E-4
EP-m kg N eqv. 3.90E-3 2.50E-4 3.83E-3 3.51E-4 4.42E-4 0.00E+0 5.30E-5 4.13E-4 2.50E-5 -4.96E-4
EP-fw kg P eqv. 1.08E-3 1.35E-7 2.59E-4 1.42E-6 6.78E-5 0.00E+0 2.62E-7 1.01E-5 8.50E-8 -4.86E-6
EP-T mol N eqv. 4.08E-2 2.78E-3 4.27E-2 3.91E-3 4.79E-3 0.00E+0 5.84E-4 4.61E-3 1.52E-4 -5.46E-3
kg CFC 11
ODP 2.04E-7 6.41E-9 3.18E-7 2.57E-8 3.39E-8 0.00E+0 5.72E-9 1.03E-7 1.46E-9 -2.06E-7
eqv.
kg NMVOC
POCP 1.55E-2 7.21E-4 1.29E-2 1.07E-3 1.59E-3 0.00E+0 1.67E-4 1.24E-3 5.82E-5 -2.01E-3
eqv.
AP=Acidification (AP) | GWP-total=Global warming potential (GWP-total) | GWP-b=Global warming potential - Biogenic (GWP-b) | GWP-f=Global warming potential - Fossil (GWP-f) | GWP-
luluc=Global warming potential - Land use and land use change (GWP-luluc) | EP-m=Eutrophication marine (EP-m) | EP-fw=Eutrophication, freshwater (EP-fw) | EP-T=Eutrophication,
terrestrial (EP-T) | ODP=Ozone depletion (ODP) | POCP=Photochemical ozone formation - human health (POCP) | ADP-f=Resource use, fossils (ADP-f) | ADP-mm=Resource use, minerals and
metals (ADP-mm) | WDP=Water use (WDP)
ACEFormer™ | ReTHiNK-58053 15 / 24
Environmental Product Declaration
5 Results
Abbreviation Unit A1 A2 A3 A4 A5 C1 C2 C3 C4 D
ADP-f MJ 1.35E+2 4.09E-1 9.59E+1 1.78E+0 1.19E+1 0.00E+0 3.91E-1 2.62E+0 1.12E-1 -3.25E+1
ADP-mm kg Sb-eqv. 6.52E-5 2.51E-7 1.08E-5 2.11E-6 4.17E-6 0.00E+0 6.57E-7 4.30E-6 5.07E-8 -2.09E-6
m3 world
WDP 1.96E+0 6.23E-4 9.49E-1 7.81E-3 1.55E-1 0.00E+0 1.40E-3 1.71E-1 4.80E-3 -2.63E-1
eqv.
AP=Acidification (AP) | GWP-total=Global warming potential (GWP-total) | GWP-b=Global warming potential - Biogenic (GWP-b) | GWP-f=Global warming potential - Fossil (GWP-f) | GWP-
luluc=Global warming potential - Land use and land use change (GWP-luluc) | EP-m=Eutrophication marine (EP-m) | EP-fw=Eutrophication, freshwater (EP-fw) | EP-T=Eutrophication,
terrestrial (EP-T) | ODP=Ozone depletion (ODP) | POCP=Photochemical ozone formation - human health (POCP) | ADP-f=Resource use, fossils (ADP-f) | ADP-mm=Resource use, minerals and
metals (ADP-mm) | WDP=Water use (WDP)
ADDITIONAL ENVIRONMENTAL IMPACT INDICATORS EN15084+A2
Abbreviation Unit A1 A2 A3 A4 A5 C1 C2 C3 C4 D
ETP-fw CTUe 6.49E+1 2.66E-1 7.27E+1 1.47E+0 9.10E+0 0.00E+0 3.49E-1 4.22E+1 1.19E-1 -2.55E+0
disease
PM 1.80E-7 1.03E-9 7.52E-8 8.53E-9 1.40E-8 0.00E+0 2.33E-9 1.23E-8 7.80E-10 -9.18E-9
incidence
HTP-c CTUh 1.61E-9 1.80E-11 1.41E-9 4.81E-11 1.88E-10 0.00E+0 1.13E-11 6.43E-10 3.13E-12 -1.47E-10
HTP-nc CTUh 4.22E-8 2.16E-10 4.90E-8 1.49E-9 5.34E-9 0.00E+0 3.81E-10 1.33E-8 7.76E-11 -2.53E-9
IR kBq U235 eqv. 2.29E-1 1.75E-3 2.77E-1 7.60E-3 2.65E-2 0.00E+0 1.64E-3 1.07E-2 4.39E-4 -1.28E-2
SQP Pt 8.50E+0 6.39E-2 9.22E+0 1.13E+0 1.03E+0 0.00E+0 3.39E-1 9.63E-1 2.65E-1 -5.89E-1
ETP-fw=Ecotoxicity, freshwater (ETP-fw) | PM=Particulate Matter (PM) | HTP-c=Human toxicity, cancer (HTP-c) | HTP-nc=Human toxicity, non-cancer (HTP-nc) | IR=Ionising radiation, human
health (IR) | SQP=Land use (SQP)
CLASSIFICATION OF DISCLAIMERS TO THE DECLARATION OF CORE AND ADDITIONAL ENVIRONMENTAL IMPACT INDICATORS
ILCD classification Indicator Disclaimer
Global warming potential (GWP) None
ILCD type / level 1 Depletion potential of the stratospheric ozone layer (ODP) None
Potential incidence of disease due to PM emissions (PM) None
AAcidification potential, Accumulated Exceedance (AP) None
ILCD type / level 2
None
ACEFormer™ | ReTHiNK-58053 16 / 24
Environmental Product Declaration
5 Results
ILCD classification Indicator Disclaimer
Eutrophication potential, Fraction of nutrients reaching freshwater end compartment
(EP-freshwater)
Eutrophication potential, Fraction of nutrients reaching marine end compartment
None
(EP-marine)
Eutrophication potential, Accumulated Exceedance (EP-terrestrial) None
Formation potential of tropospheric ozone (POCP) None
Potential Human exposure efficiency relative to U235 (IRP) 1
Abiotic depletion potential for non-fossil resources (ADP-minerals&metals) 2
Abiotic depletion potential for fossil resources (ADP-fossil) 2
Water (user) deprivation potential, deprivation-weighted water consumption (WDP) 2
ILCD type / level 3 Potential Comparative Toxic Unit for ecosystems (ETP-fw) 2
Potential Comparative Toxic Unit for humans (HTP-c) 2
Potential Comparative Toxic Unit for humans (HTP-nc) 2
Potential Soil quality index (SQP) 2
Disclaimer 1 – This impact category deals mainly with the eventual impact of low dose ionizing radiation on human health of the nuclear fuel cycle. It does not consider effects due to possible
nuclear accidents, occupational exposure nor due to radioactive waste disposal in underground facilities. Potential ionizing radiation from the soil, from radon and from some construction
materials is also not measured by this indicator.
Disclaimer 2 – The results of this environmental impact indicator shall be used with care as the uncertainties on these results are high or as there is limited experienced with the indicator.
ACEFormer™ | ReTHiNK-58053 17 / 24
Environmental Product Declaration
5 Results
5.3 ENVIRONMENTAL IMPACT INDICATORS PER SQUARE METER (FIXED PART)
PARAMETERS DESCRIBING RESOURCE USE
Abbreviation Unit A1 A2 A3 A4 A5 C1 C2 C3 C4 D
PERE MJ -5.77E-1 -5.88E-4 -6.28E-1 -5.33E-3 -6.16E-2 5.07E-3 -1.01E-3 -5.49E-2 -4.11E-4 6.91E-3
PERM MJ 0.00E+0 0.00E+0 0.00E+0 0.00E+0 0.00E+0 0.00E+0 0.00E+0 0.00E+0 0.00E+0 0.00E+0
PERT MJ -5.77E-1 -5.88E-4 -6.28E-1 -5.33E-3 -6.16E-2 5.07E-3 -1.01E-3 -5.49E-2 -4.11E-4 6.91E-3
PENRE MJ -1.92E+1 -9.26E-2 -1.59E+1 -3.79E-1 -1.81E+0 9.95E-1 -8.60E-2 -5.76E-1 -2.47E-2 6.54E+0
PENRM MJ -1.08E+1 0.00E+0 -1.16E-1 0.00E+0 -5.47E-1 0.00E+0 0.00E+0 0.00E+0 0.00E+0 8.12E-1
PENRT MJ -3.00E+1 -9.26E-2 -1.60E+1 -3.79E-1 -2.36E+0 9.95E-1 -8.60E-2 -5.76E-1 -2.47E-2 7.36E+0
SM Kg 0.00E+0 0.00E+0 0.00E+0 0.00E+0 0.00E+0 0.00E+0 0.00E+0 0.00E+0 0.00E+0 0.00E+0
RSF MJ 0.00E+0 0.00E+0 0.00E+0 0.00E+0 0.00E+0 0.00E+0 0.00E+0 0.00E+0 0.00E+0 0.00E+0
NRSF MJ 0.00E+0 0.00E+0 0.00E+0 0.00E+0 0.00E+0 0.00E+0 0.00E+0 0.00E+0 0.00E+0 0.00E+0
FW M3 -1.04E-2 -4.54E-6 -4.29E-3 -5.14E-5 -7.59E-4 4.83E-5 -9.87E-6 -1.04E-3 -2.43E-5 7.70E-4
PERE=renewable primary energy ex. raw materials | PERM=renewable primary energy used as raw materials | PERT=renewable primary energy total | PENRE=non-renewable primary energy
ex. raw materials | PENRM=non-renewable primary energy used as raw materials | PENRT=non-renewable primary energy total | SM=use of secondary material | RSF=use of renewable
secondary fuels | NRSF=use of non-renewable secondary fuels | FW=use of net fresh water
OTHER ENVIRONMENTAL INFORMATION DESCRIBING WASTE CATEGORIES
Abbreviation Unit A1 A2 A3 A4 A5 C1 C2 C3 C4 D
HWD Kg -1.77E-5 -7.97E-8 -6.39E-6 -7.09E-7 -1.28E-6 2.55E-6 -2.05E-7 -1.03E-6 -3.53E-8 6.90E-6
NHWD Kg -6.99E-2 -2.02E-4 -5.88E-2 -1.55E-2 -1.12E-2 1.11E-3 -5.14E-3 -1.34E-2 -9.28E-2 3.33E-3
RWD Kg -1.85E-5 -6.07E-7 -3.83E-5 -2.34E-6 -3.04E-6 6.51E-6 -5.32E-7 -1.95E-6 -1.38E-7 3.34E-6
HWD=hazardous waste disposed | NHWD=non hazardous waste disposed | RWD=radioactive waste disposed
ACEFormer™ | ReTHiNK-58053 18 / 24
Environmental Product Declaration
5 Results
ENVIRONMENTAL INFORMATION DESCRIBING OUTPUT FLOWS
Abbreviation Unit A1 A2 A3 A4 A5 C1 C2 C3 C4 D
CRU Kg 0.00E+0 0.00E+0 0.00E+0 0.00E+0 0.00E+0 0.00E+0 0.00E+0 0.00E+0 0.00E+0 0.00E+0
MFR Kg 0.00E+0 0.00E+0 -4.50E-8 0.00E+0 1.91E-3 0.00E+0 0.00E+0 -1.85E-2 0.00E+0 0.00E+0
MER Kg 0.00E+0 0.00E+0 0.00E+0 0.00E+0 0.00E+0 0.00E+0 0.00E+0 0.00E+0 0.00E+0 0.00E+0
EET MJ 0.00E+0 0.00E+0 -1.68E-1 0.00E+0 0.00E+0 0.00E+0 0.00E+0 0.00E+0 0.00E+0 -2.37E+0
EEE MJ 0.00E+0 0.00E+0 -9.74E-2 0.00E+0 0.00E+0 0.00E+0 0.00E+0 0.00E+0 0.00E+0 -1.37E+0
CRU=Components for re-use | MFR=Materials for recycling | MER=Materials for energy recovery | EET=Exported Energy Thermic | EEE=Exported Energy Electric
5.4 ENVIRONMENTAL IMPACT INDICATORS PER SQUARE METER (SCALABLE PART)
PARAMETERS DESCRIBING RESOURCE USE
Abbreviation Unit A1 A2 A3 A4 A5 C1 C2 C3 C4 D
PERE MJ 2.71E+0 2.83E-3 3.98E+0 2.66E-2 3.50E-1 0.00E+0 4.90E-3 2.65E-1 1.98E-3 -1.66E-1
PERM MJ 0.00E+0 0.00E+0 0.00E+0 0.00E+0 0.00E+0 0.00E+0 0.00E+0 0.00E+0 0.00E+0 0.00E+0
PERT MJ 2.71E+0 2.83E-3 3.98E+0 2.66E-2 3.50E-1 0.00E+0 4.90E-3 2.65E-1 1.98E-3 -1.66E-1
PENRE MJ 9.29E+1 4.35E-1 9.93E+1 1.89E+0 9.99E+0 0.00E+0 4.15E-1 2.78E+0 1.19E-1 -3.18E+1
PENRM MJ 5.16E+1 0.00E+0 2.56E+0 0.00E+0 2.71E+0 0.00E+0 0.00E+0 0.00E+0 0.00E+0 -3.99E+0
PENRT MJ 1.44E+2 4.35E-1 1.02E+2 1.89E+0 1.27E+1 0.00E+0 4.15E-1 2.78E+0 1.19E-1 -3.58E+1
SM Kg 0.00E+0 0.00E+0 0.00E+0 0.00E+0 0.00E+0 0.00E+0 0.00E+0 0.00E+0 0.00E+0 0.00E+0
RSF MJ 0.00E+0 0.00E+0 0.00E+0 0.00E+0 0.00E+0 0.00E+0 0.00E+0 0.00E+0 0.00E+0 0.00E+0
NRSF MJ 0.00E+0 0.00E+0 0.00E+0 0.00E+0 0.00E+0 0.00E+0 0.00E+0 0.00E+0 0.00E+0 0.00E+0
FW M3 4.95E-2 2.21E-5 2.70E-2 2.56E-4 4.11E-3 0.00E+0 4.76E-5 5.03E-3 1.17E-4 -3.77E-3
PERE=renewable primary energy ex. raw materials | PERM=renewable primary energy used as raw materials | PERT=renewable primary energy total | PENRE=non-renewable primary energy
ex. raw materials | PENRM=non-renewable primary energy used as raw materials | PENRT=non-renewable primary energy total | SM=use of secondary material | RSF=use of renewable
secondary fuels | NRSF=use of non-renewable secondary fuels | FW=use of net fresh water
ACEFormer™ | ReTHiNK-58053 19 / 24
Environmental Product Declaration
5 Results
OTHER ENVIRONMENTAL INFORMATION DESCRIBING WASTE CATEGORIES
Abbreviation Unit A1 A2 A3 A4 A5 C1 C2 C3 C4 D
HWD Kg 8.19E-5 3.93E-7 4.01E-5 3.54E-6 6.72E-6 0.00E+0 9.91E-7 4.99E-6 1.70E-7 -3.35E-5
NHWD Kg 3.29E-1 1.67E-3 3.67E-1 7.74E-2 6.56E-2 0.00E+0 2.48E-2 6.45E-2 4.48E-1 -1.64E-2
RWD Kg 1.02E-4 2.84E-6 2.39E-4 1.17E-5 1.84E-5 0.00E+0 2.57E-6 9.40E-6 6.66E-7 -1.63E-5
HWD=hazardous waste disposed | NHWD=non hazardous waste disposed | RWD=radioactive waste disposed
ENVIRONMENTAL INFORMATION DESCRIBING OUTPUT FLOWS
Abbreviation Unit A1 A2 A3 A4 A5 C1 C2 C3 C4 D
CRU Kg 0.00E+0 0.00E+0 0.00E+0 0.00E+0 0.00E+0 0.00E+0 0.00E+0 0.00E+0 0.00E+0 0.00E+0
MFR Kg 0.00E+0 0.00E+0 3.75E-4 0.00E+0 4.49E-3 0.00E+0 0.00E+0 8.94E-2 0.00E+0 0.00E+0
MER Kg 0.00E+0 0.00E+0 0.00E+0 0.00E+0 0.00E+0 0.00E+0 0.00E+0 0.00E+0 0.00E+0 0.00E+0
EET MJ 0.00E+0 0.00E+0 7.80E-1 0.00E+0 0.00E+0 0.00E+0 0.00E+0 0.00E+0 0.00E+0 1.15E+1
EEE MJ 0.00E+0 0.00E+0 4.53E-1 0.00E+0 0.00E+0 0.00E+0 0.00E+0 0.00E+0 0.00E+0 6.68E+0
CRU=Components for re-use | MFR=Materials for recycling | MER=Materials for energy recovery | EET=Exported Energy Thermic | EEE=Exported Energy Electric
ACEFormer™ | ReTHiNK-58053 20 / 24
Environmental Product Declaration
5 Results
5.5 INFORMATION ON BIOGENIC CARBON CONTENT PER SQUARE METER
BIOGENIC CARBON CONTENT
The following Information describes the biogenic carbon content in (the main parts of) the
product at the factory gate per square meter:
Biogenic carbon content Amount Unit
Biogenic carbon content in the product 0 kg C
Biogenic carbon content in accompanying packaging 0 kg C
ACEFormer™ | ReTHiNK-58053 21 / 24
Environmental Product Declaration
6 Interpretation of results
As shown in the figure below, the production process (A3) and raw material supply (A1)
dominate in most environmental core indicators. The highest influence on the Global
Warming Potential (GWP-total) have production process (A3) and waste processing (C3) .
Transports (A2, C2) have rather a minor impact within all core indicators.
ACEFormer™ | ReTHiNK-58053 22 / 24
Environmental Product Declaration
7 References
ISO 14040
ISO 14040:2006-10, Environmental management - Life cycle assessment - Principles and
framework; EN ISO 14040:2006
ISO 14044
ISO 14044:2006-10, Environmental management - Life cycle assessment - Requirements
and guidelines; EN ISO 14040:2006
ISO 14025
ISO 14025:2011-10: Environmental labels and declarations — Type III environmental
declarations — Principles and procedures
EN 15804+A2
EN 15804+A2: 2019: Sustainability of construction works — Environmental Product
Declarations — Core rules for the product category of construction products
PCR A: General Program Category Rules for Construction Products from the EPD program
Kiwa-Ecobility Experts, 2022-02-14
PCR B: Product Category Rules (PCR) from the Kiwa-Ecobility Experts (Kiwa-EE) – Specific
Product Category Rules: Geosynthetic products, 2023-07-21
ACEFormer™ | ReTHiNK-58053 23 / 24
Environmental Product Declaration
8 Contact information
Publisher Operator Owner of declaration
Kiwa-Ecobility Experts Kiwa-Ecobility Experts Gold-Joint Industry Co., Ltd.
Voltastraße 5 Voltastraße 5 No.33, Jing 3 Rd. Wuqi Dist.
13355 Berlin, DE 13355 Berlin, DE 43541 Taichung City, Taiwan (R.O.C.), TW
E-mail: E-mail: E-mail:
DE.Ecobility.Experts@kiwa.com DE.Ecobility.Experts@kiwa.com marketing@geoace.com
Website: Website: Website:
https://www.kiwa.com/de/en/themes/ecobility-experts/ecobility-https://www.kiwa.com/de/en/themes/ecobility-experts/ecobility-www.geoace.com
experts-epd-program/ experts-epd-program/
Kiwa-Ecobility Experts is
established member of the
ACEFormer™ | ReTHiNK-58053 24 / 24
