ENVIRONMENTAL PRODUCT DECLARATION
as per ISO 14025 and EN 15804+A2
Owner of the Declaration Balsan
Programme holder Institut Bauen und Umwelt e.V. (IBU)
Publisher Institut Bauen und Umwelt e.V. (IBU)
Declaration number EPD-BAL-20220233-CCA1-EN
Issue date 18.08.2022
Valid to 17.08.2027
PILOTE 3D NRB (Noise Reduction Backing)
tufted carpet tiles made of recycled material
Balsan
www.ibu-epd.com | https://epd-online.com
Umwelt Produktdeklaration Name des Herstellers – Name des Produkts
General Information
Balsan PILOTE 3D NRB - tufted carpet tiles
made of recycled material
Programme holder Owner of the declaration
IBU – Institut Bauen und Umwelt e.V. Balsan
Hegelplatz 1 Corbilly - D14
10117 Berlin 36330 Arthon
Germany France
Declaration number Declared product / declared unit
EPD-BAL-20220233-CCA1-EN 1 m2 tufted carpet tiles PILOTE 3D NRB
This declaration is based on the product Scope:
category rules: The manufacturer declaration applies to the tufted
Floor coverings, 02/2018 carpet tiles PILOTE 3D NRB with the GUT- PRODIS
(PCR checked and approved by the SVR) license number 06791FF8.
The products are produced in the Balsan
manufacturing sites Arthon (tufting and precoating) and
Issue date
Neuvy-Saint-Sépulchre (back coating), France.
18.08.2022
The declaration is only valid in conjunction with a valid
GUT-PRODIS license of the product.
Valid to
17.08.2027
The owner of the declaration shall be liable for the
underlying information and evidence; the IBU shall not
be liable with respect to manufacturer information, life
cycle assessment data and evidences.
The EPD was created according to the specifications
of EN 15804+A2. In the following, the standard will be
simplified as EN 15804.
Verification
The standard EN 15804 serves as the core PCR
Independent verification of the declaration and data
according to ISO 14025:2011
Dipl. Ing. Hans Peters internally x externally
(chairman of Institut Bauen und Umwelt e.V.)
Dr. Alexander Röder Angela Schindler
(Managing Director Institut Bauen und Umwelt e.V.)) (Independent verifier)
Product
Product description/Product definition For the application and use of the product the
PILOTE 3D NRB (Noise Reduction Backing) - tufted respective national provisions apply.
carpet tiles having a surface pile of solution-dyed
polyamide 6 with 100% recycled content, a polyester Application
primary backing with 90% recycled content and a According to the use class as defined in EN 1307 the
bitumen based heavy backing with a fibre glass products can be used in all professional areas which
reinforcement and a polyester covering fleece made of require class 33 or less.
85% recycled material.
The total recycled content amounts to 25%.
For the placing on the market of the product in the
European Union/European Free Trade Association
(EU/EFTA) (with the exception of Switzerland)
Regulation (EU) No. 305/2011 Construction Product
Regulation (CPR) applies. The product needs a
Declaration of Performance (DoP) taking into
consideration EN 14041:2018-05, Resilient, textile and
laminate floor coverings - Essential characteristics, and
the CE-marking. The DoP of the product can be found
on the manufacturer's technical information section.
2 Environmental Product Declaration Balsan – PILOTE 3D NRB - tufted carpet tiles
Technical Data Base materials/Ancillary materials
Name Value Unit
Constructional data Polyamide 6 16.2 %
Name Value Unit Polyester 10.2 %
Product Form Tiles 50 cm x 50 cm - SBR-latex 4.2 %
Type of manufacture Tufted carpet tiles - Limestone 54.5 %
Polyamide 6, Bitumen 14.0 %
Yarn type -
100 % recycled Glass fibre 0.9 %
Coloration Solution dyed yarn This product contains substances listed in the ECHA
Primary backing Polyester, 90 % recycled candidate list (10.06.2022) or other carcinogenic,
Bitumen based heavy mutagenic or reprotoxic (CMR) substances in
Secondary backing backing with a 85 % - categories 1A or 1B which are not on the candidate list
recycled polyester fleece exceeding 0.1 percentage by mass: no
Surface pile weight 420 g/m2 The products are registered in the GUT-PRODIS
Surface pile thickness 3.8 mm Information System. The PRODIS system ensures the
Total pile weight 620 g/m² compliance with limitations of various chemicals and
Total carpet weight 3835 g/m2 Volatile Organic Compound (VOC)-emissions and a
Total thickness 8 mm ban on the use of all substances that are listed as
Number of tufts or 'Substances of Very High Concern' (SVHC) under
loops 1738 pce/dm2 REACH.
Reference service life
Performance data of the product in accordance with The service life of textile floor coverings strongly
the declaration of performance with respect to its depends on the correct installation taking into account
essential characteristics according to EN 14041: 2018- the declared use classification and the adherence to
05, Resilient, textile and laminate floor coverings - cleaning and maintenance instructions.
Essential characteristics. A calculation of the reference service life according to
ISO 15686 is not possible.
Additional product properties in accordance with EN
Alternatively, a reference service life of 10 years can
1307 can be found on the Product Information System
be assumed, during which the functional and visual
PRODIS using the PRODIS registration number of the
quality is guaranteed (BNB, Nutzungsdauer von
product (www.pro-dis.info) or on the manufacturer's
Bauteilen). The technical service life can be
technical information section (www.balsan.com).
significantly longer.
LCA: Calculation rules
Declared Unit emissions, waste water treatment, packaging material
and waste processing up to the landfill disposal of
residual waste (except radioactive waste). Benefits for
Name Value Unit generated electricity and steam due to the incineration
Declared unit 1 m2 of production waste are aggregated.
Grammage 3.835 kg/m2 Biogenic carbon that is stored in renewable material
Layer thickness 0.008 m (packaging paper) is taken into account as well as the
Gross density 479 kg/m3 associated carbon dioxide uptake from the air from
The declared unit refers to 1 m2 produced textile floor which this biogenic carbon originates.
covering. The output of module A5 'Assembly' is 1 m2
installed textile floor covering. A4 Transport
Transport of the packed textile floor covering from
factory gate to the place of installation.
System boundary
Type of EPD A5 Installation
Cradle-to-gate with options, module C1-C4, module D, Installation of the textile floor covering, processing of
and additional modules A4, A5, B1, B2 installation waste and packaging waste up to the
landfill disposal of residual waste (except radioactive
System boundaries of modules A, B, C, D waste), the production of the amount of carpet that
Modules C3, C4 and D are indicated separately for occurs as installation waste including its transport to
three end-of-life scenarios: the place of installation.
1 - landfill disposal Generated electricity and steam due to the incineration
2 - municipal waste incineration of waste are listed in the result table as exported
3 - recovery in a cement plant energy.
Biogenic carbon that is stored in renewable materials
A1-A3 Production in packaging paper is released as carbon dioxide
Energy supply and production of the basic material, emissions into the air at the end of life in module A5.
processing of secondary material, auxiliary material, Preparation of the floor and auxiliary materials
transport of the material to the manufacturing site, (adhesives, fixing agents, PET connectors) are beyond
the system boundaries and not taken into account.
3 Environmental Product Declaration Balsan – PILOTE 3D NRB - tufted carpet tiles
the result table as exported energy.
B1 Use C3-3: Collection of the carpet waste for recovery in the
Indoor emissions during the use stage. After the first cement industry, waste processing (granulating),
year, no product-related Volatile Organic Compound transport to the cement plant, emissions from the
(VOC) emissions are relevant due to known VOC incineration.
decay curves of the product.
C4 Disposal
B2 Maintenance C4-1: Impact from landfill disposal,
Cleaning of the textile floor covering for a period of 1 C4-2: The carpet waste leaves the system in module
year: C3-2,
Vacuum cleaning – electricity supply C4-3: The pre-processed carpet waste leaves the
Wet cleaning – electricity, water consumption, system in module C3-3.
production of the cleaning agent, waste water
treatment. D Recycling potential
The declared values in this module have to be Calculated benefits result from materials exclusive
multiplied by the assumed service life of the floor secondary materials (net materials).
covering in the building in question. D-A5: Benefits for generated energy due
to incineration of packaging and installation waste
B3 - B5 Repair, replacement, refurbishment (incineration plant with R1 > 0.6),
The modules are not relevant within the assumed D-1: Benefits for generated energy due to landfill
reference service life of 10 years. disposal of carpet waste at the end of life,
D-2: Benefits for generated energy due to incineration
B6 - B7 Operational energy and water use of carpet waste at the end-of-life (incineration plant
No energy and water input are required for the with R1 > 0.6),
operation of the carpet in the use stage. The modules D-3: Benefits for saved fossil energy and saved
are not relevant and not declared inorganic material due to recovery of the carpet in a
cement plant.
C1 De-construction
The floor covering is de-constructed manually and no Comparability
additional environmental impact is caused. Basically, a comparison or an evaluation of EPD data
is only possible if all the data sets to be compared
C2 Transport were created according to EN 15804 and the building
Transport of the carpet waste to a landfill, to the context, respectively the product-specific
municipal waste incineration plant (MWI) or to the characteristics of performance, are taken into account.
waste collection facility for recycling.
Background data are taken from the GaBi database,
C3 Waste processing 2022-1. Remaining data gaps are covered by the
C3-1: Landfill disposal needs no waste processing. ecoinvent 3.7 database, 2020.
C3-2: Impact from waste incineration (plant with
R1>0.6), generated electricity and steam are listed in
LCA: Scenarios and additional technical information
Characteristic product properties Preparation of the floor and auxiliaries (adhesives,
Information on biogenic Carbon fixing agents, PET connectors etc.) are not taken into
account.
Name Value Unit Maintenance (B2)
Biogenic Carbon Content in The values for cleaning refer to 1 m2 floor covering per
0.04 kg C
accompanying packaging year.
1 kg biogenic Carbon is equivalent to 44/12 kg of CO Depending on the application based on ISO 10874, the
2
technical service life recommended by the
manufacturer and the anticipated strain on the floor by
customers, the case-specific useful life can be
established. Based on this useful life the effects of
Transport to the construction site (A4) module B2 need to be calculated in order to obtain the
Name Value Unit overall environmental impacts.
Litres of fuel 0.009 l/100km Name Value Unit
Transport distance 700 km Number/
Maintenance cycle (vacuum cleaning) 208
Capacity utilisation (including empty year
55 %
runs) Number/
Maintenance cycle (wet cleaning) 1,5
Gross density of products transported 479 kg/m3 year
Water consumption (wet cleaning) 4,4 kg/year
Installation in the building (A5) Cleaning agent (wet cleaning) 0,09 kg/year
Name Value Unit Electricity consumption 0,314 kWh/year
Material loss 0.115 kg
Polyethylene packaging waste and installation waste
are considered to be incinerated in a municipal waste
incineration plant. Cardboard packaging waste is going
to be recycled.
4 Environmental Product Declaration Balsan – PILOTE 3D NRB - tufted carpet tiles
Reference service life
Name Value Unit
Life Span (according to BBSR) 10 a
Corresponds to the
Declared product properties
specifications of EN -
(at the gate) and finishes
1307
An assumed quality of work,
Conforms to the
when installed in accordance
manufacturer's -
with the manufacturer’s
instructions
instructions
Use in areas
Usage conditions, e.g.
corresponding to use
frequency of use, mechanical -
class 33 according to
exposure
EN 1307
Maintenance e.g. required
According to the
frequency, type and quality
manufacturers -
and replacement of
instructions
components
End of Life (C1-C4)
Three different end of life scenarios are declared and
the results are indicated separately in module C.
Each scenario is calculated as a 100% scenario.
Scenario 1: 100 % landfill disposal
Scenario 2: 100 % municipal waste incineration (MWI)
with R1>0.6
Scenario 3: 100 % recovery in the cement industry
If combinations of these scenarios have to be
calculated this should be done according to the
following scheme:
EOL-impact = x % impact (Scenario 1)
+ y % impact (Scenario 2)
+ z % impact (Scenario 3)
with x % + y % + z % = 100 %
Name Value Unit
Collected as mixed construction
3.835 kg
waste (scenario 1 and 2)
Collected separately (scenario 3) 3.835 kg
Landfilling (scenario 1) 3.835 kg
Energy recovery (scenario 2) 3.835 kg
Energy recovery (scenario 3) 1.708 kg
Recycling (scenario 3) 2.127 kg
Reuse, recovery and/or recycling potentials (D),
relevant scenario information
Recovery or recycling potentials due to the three end
of life scenarios (module C) are indicated separately.
Recycling in the cement industry (scenario 3)
The organic material of the carpet is used as an
alternative fuel in a cement kiln. It mainly substitutes
for lignite (68.8 %), hard coal (23.6 %) and petrol coke
(7.6 %). The inorganic material is substantially
integrated into the cement clinker and substitutes for
original material input VDZ e.V.
5 Environmental Product Declaration Balsan – PILOTE 3D NRB - tufted carpet tiles
LCA: Results
The modules C3/1, C4/2 and C4/3 cause no additional impact (see chapter "LCA: Calculation rules").
Module C2 represents the transport for scenarios 1, 2 and 3. The values in column D result from module A5.
DESCRIPTION OF THE SYSTEM BOUNDARY (X = INCLUDED IN LCA; ND = MODULE OR INDICATOR NOT
DECLARED; MNR = MODULE NOT RELEVANT)
BENEFITS AND
CONSTRUCTI LOADS
PRODUCT STAGE ON PROCESS USE STAGE END OF LIFE STAGE BEYOND THE
STAGE SYSTEM
BOUNDARIES
6 Environmental Product Declaration Balsan – PILOTE 3D NRB - tufted carpet tiles
lairetam
waR
ylppus tropsnarT
gnirutcafunaM
eht
morf
tropsnarT
etis
eht
ot
etag
ylbmessA esU
ecnanetniaM
riapeR
tnemecalpeR tnemhsibrufeR
ygrene
lanoitarepO esu
retaw
lanoitarepO esu
noitcurtsnoc-eD
noitilomed tropsnarT
gnissecorp
etsaW
lasopsiD -esueR -yrevoceR -gnilcyceR laitnetop
A1 A2 A3 A4 A5 B1 B2 B3 B4 B5 B6 B7 C1 C2 C3 C4 D
X X X X X X X MNR MNR MNR ND ND X X X X X
RESULTS OF THE LCA - ENVIRONMENTAL IMPACT according to EN 15804+A2: 1 m² floor covering
Core Indicator Unit A1-A3 A4 A5 B1 B2 C1 C2 C3/2 C3/3 C4/1 D D/1 D/2 D/3
GWP-total [kg CO2-Eq.] 3.85E+02.33E-1 4.09E-10.00E+04.16E-10.00E+01.30E-24.53E+04.59E+02.69E-1-1.08E-20.00E+0-3.11E-1-1.61E-1
GWP-fossil [kg CO2-Eq.] 4.07E+02.29E-1 2.68E-10.00E+02.15E-10.00E+01.28E-24.53E+04.59E+02.69E-1-1.08E-20.00E+0-3.10E-1-1.61E-1
GWP-biogenic [kg CO2-Eq.] -2.23E-12.97E-3 1.40E-10.00E+04.16E-30.00E+01.65E-4 5.76E-4 1.17E-3 3.25E-8-5.21E-50.00E+0-1.49E-37.11E-5
GWP-luluc [kg CO2-Eq.] 4.78E-3 1.30E-3 1.92E-40.00E+01.96E-10.00E+07.24E-5 2.18E-4 4.03E-4 1.32E-4-1.11E-60.00E+0-3.14E-5-8.28E-5
1.39E- 2.19E- 7.78E- 3.32E- 6.21E- 3.65E- -6.68E- -1.89E- -3.28E-
ODP [kg CFC11-Eq.] 7.28E-9 0.00E+03.42E-80.00E+0 0.00E+0
14 10 16 13 13 13 14 12 13
AP [mol H+-Eq.] 1.23E-2 1.39E-3 5.16E-40.00E+08.32E-40.00E+07.73E-5 3.42E-3 3.65E-3 8.06E-4-1.35E-50.00E+0-3.85E-4-4.92E-4
EP-freshwater [kg P-Eq.] 3.38E-5 6.95E-7 1.06E-60.00E+05.19E-60.00E+03.87E-8 7.57E-7 9.12E-7 5.07E-5-1.36E-80.00E+0-3.87E-7-2.39E-7
EP-marine [kg N-Eq.] 4.17E-3 6.80E-4 1.96E-40.00E+01.97E-40.00E+03.79E-5 1.63E-3 1.74E-3 1.78E-4-3.74E-60.00E+0-1.07E-4-1.68E-4
EP-terrestrial [mol N-Eq.] 3.95E-2 7.53E-3 1.98E-30.00E+02.83E-30.00E+04.20E-4 1.83E-2 1.95E-2 1.96E-3-4.01E-50.00E+0-1.15E-3-1.85E-3
POCP [kg NMVOC-Eq.]1.05E-2 1.29E-3 4.84E-4 4.18E-4 9.83E-40.00E+07.17E-5 4.20E-3 4.41E-3 5.73E-4-1.05E-50.00E+0-3.01E-4-5.19E-4
ADPE [kg Sb-Eq.] 8.59E-7 1.95E-8 2.71E-80.00E+02.30E-70.00E+01.09E-9 2.23E-8 3.04E-8 1.89E-8-1.53E-90.00E+0-4.36E-8-1.75E-8
- -
ADPF [MJ] 8.16E+13.11E+02.63E+00.00E+05.90E+00.00E+01.74E-12.57E+03.36E+03.86E+0-1.82E-10.00E+0
5.24E+02.27E+1
[m³ world-Eq
WDP 3.83E+02.08E-3 1.33E-10.00E+09.99E-20.00E+01.16E-4 6.06E-1 6.10E-1-2.88E-3-1.04E-30.00E+0-2.95E-2-2.12E-2
deprived]
GWP = Global warming potential; ODP = Depletion potential of the stratospheric ozone layer; AP = Acidification potential of land and water; EP =
Caption Eutrophication potential; POCP = Formation potential of tropospheric ozone photochemical oxidants; ADPE = Abiotic depletion potential for non-
fossil resources; ADPF = Abiotic depletion potential for fossil resources; WDP = Water (user) deprivation potential
RESULTS OF THE LCA - INDICATORS TO DESCRIBE RESOURCE USE according to EN 15804+A2: 1 m²
floor covering
Indicator Unit A1-A3 A4 A5 B1 B2 C1 C2 C3/2 C3/3 C4/1 D D/1 D/2 D/3
PERE [MJ] 3.98E+1 1.77E-1 1.40E+0 0.00E+0 3.69E+0 0.00E+0 9.86E-3 4.47E-1 6.70E-1 3.17E-1 -4.62E-2 0.00E+0 -1.31E+0-1.98E-1
PERM [MJ] 1.79E-1 0.00E+0 -1.79E-1 0.00E+0 0.00E+0 0.00E+0 0.00E+0 0.00E+0 0.00E+0 0.00E+0 0.00E+0 0.00E+0 0.00E+0 0.00E+0
PERT [MJ] 4.00E+1 1.77E-1 1.22E+0 0.00E+0 3.69E+0 0.00E+0 9.86E-3 4.47E-1 6.70E-1 3.17E-1 -4.62E-2 0.00E+0 -1.31E+0-1.98E-1
PENRE [MJ] 5.64E+1 3.12E+0 2.67E+0 0.00E+0 5.90E+0 0.00E+0 1.74E-1 2.79E+1 2.87E+1 3.86E+0 -1.82E-1 0.00E+0 -5.24E+0-2.27E+1
PENRM [MJ] 2.54E+1 0.00E+0 -4.30E-2 0.00E+0 0.00E+0 0.00E+0 0.00E+0 -2.53E+1-2.53E+1 0.00E+0 0.00E+0 0.00E+0 0.00E+0 0.00E+0
PENRT [MJ] 8.18E+1 3.12E+0 2.63E+0 0.00E+0 5.90E+0 0.00E+0 1.74E-1 2.57E+0 3.36E+0 3.86E+0 -1.82E-1 0.00E+0 -5.24E+0-2.27E+1
SM [kg] 1.09E+0 0.00E+0 3.28E-2 0.00E+0 0.00E+0 0.00E+0 0.00E+0 0.00E+0 0.00E+0 0.00E+0 0.00E+0 0.00E+0 0.00E+0 1.21E+0
RSF [MJ] 0.00E+0 0.00E+0 0.00E+0 0.00E+0 0.00E+0 0.00E+0 0.00E+0 0.00E+0 0.00E+0 0.00E+0 0.00E+0 0.00E+0 0.00E+0 0.00E+0
NRSF [MJ] 0.00E+0 0.00E+0 0.00E+0 0.00E+0 0.00E+0 0.00E+0 0.00E+0 0.00E+0 0.00E+0 0.00E+0 0.00E+0 0.00E+0 0.00E+0 0.00E+0
FW [m³] 1.07E-1 2.00E-4 3.65E-3 0.00E+0 3.34E-3 0.00E+0 1.11E-5 1.43E-2 1.46E-2 4.52E-5 -4.42E-5 0.00E+0 -1.25E-3 -1.84E-3
PERE = Use of renewable primary energy excluding renewable primary energy resources used as raw materials; PERM = Use of
renewable primary energy resources used as raw materials; PERT = Total use of renewable primary energy resources; PENRE = Use of
non-renewable primary energy excluding non-renewable primary energy resources used as raw materials; PENRM = Use of non-
Caption
renewable primary energy resources used as raw materials; PENRT = Total use of non-renewable primary energy resources; SM = Use
of secondary material; RSF = Use of renewable secondary fuels; NRSF = Use of non-renewable secondary fuels; FW = Use of net fresh
water
RESULTS OF THE LCA – WASTE CATEGORIES AND OUTPUT FLOWS according to EN 15804+A2:
1 m² floor covering
Indicator Unit A1-A3 A4 A5 B1 B2 C1 C2 C3/2 C3/3 C4/1 D D/1 D/2 D/3
HWD [kg] 1.82E-3 1.49E-11 5.46E-5 0.00E+0 4.19E-5 0.00E+0 8.33E-133.78E-104.11E-105.95E-10-2.54E-110.00E+0-7.32E-10-5.17E-11
NHWD [kg] 3.10E-1 4.47E-4 4.12E-2 0.00E+0 7.30E-3 0.00E+0 2.49E-5 1.06E+0 1.06E+0 3.82E+0 -8.87E-5 0.00E+0 -2.53E-3 -5.85E-4
RWD [kg] 1.68E-3 3.84E-6 5.35E-5 0.00E+0 3.76E-4 0.00E+0 2.14E-7 9.81E-5 1.56E-4 4.74E-5 -1.32E-5 0.00E+0 -3.75E-4 -3.46E-5
CRU [kg] 0.00E+0 0.00E+0 0.00E+0 0.00E+0 0.00E+0 0.00E+0 0.00E+0 0.00E+0 0.00E+0 0.00E+0 0.00E+0 0.00E+0 0.00E+0 0.00E+0
MFR [kg] 1.41E-2 0.00E+0 9.24E-2 0.00E+0 0.00E+0 0.00E+0 0.00E+0 0.00E+0 1.21E+0 0.00E+0 0.00E+0 0.00E+0 0.00E+0 0.00E+0
MER [kg] 0.00E+0 0.00E+0 0.00E+0 0.00E+0 0.00E+0 0.00E+0 0.00E+0 0.00E+0 0.00E+0 0.00E+0 0.00E+0 0.00E+0 0.00E+0 0.00E+0
EEE [MJ] 0.00E+0 0.00E+0 1.65E-1 0.00E+0 0.00E+0 0.00E+0 0.00E+0 5.27E+0 0.00E+0 0.00E+0 0.00E+0 0.00E+0 0.00E+0 0.00E+0
EET [MJ] 0.00E+0 0.00E+0 3.09E-1 0.00E+0 0.00E+0 0.00E+0 0.00E+0 9.90E+0 5.27E+1 0.00E+0 0.00E+0 0.00E+0 0.00E+0 0.00E+0
HWD = Hazardous waste disposed; NHWD = Non-hazardous waste disposed; RWD = Radioactive waste disposed; CRU = Components
Caption for re-use; MFR = Materials for recycling; MER = Materials for energy recovery; EEE = Exported electrical energy; EET = Exported
thermal energy
RESULTS OF THE LCA – additional impact categories according to EN 15804+A2-optional:
1 m² floor covering
Indicator Unit A1-A3 A4 A5 B1 B2 C1 C2 C3/2 C3/3 C4/1 D D/1 D/2 D/3
[Disease -1.12E-
PM 1.06E-7 8.00E-9 3.99E-9 0.00E+0 6.84E-8 0.00E+04.47E-10 1.85E-8 2.00E-8 7.74E-9 0.00E+0 0.00E+0 -2.22E-8
Incidence] 10
[kBq U235-
IRP 2.80E-1 5.63E-4 8.87E-3 0.00E+0 6.78E-2 0.00E+0 3.14E-5 1.49E-2 2.47E-2 7.00E-3 -2.24E-3 0.00E+0 0.00E+0 -3.14E-3
Eq.]
ETP-fw [CTUe] 4.50E+1 2.16E+0 1.46E+0 3.60E-3 2.69E+0 0.00E+0 1.20E-1 1.38E+0 1.84E+0 3.77E+0 -3.70E-2 0.00E+0 0.00E+0-4.37E+0
-1.80E- -4.67E-
HTP-c [CTUh] 2.04E-9 4.36E-116.46E-110.00E+06.21E-100.00E+02.43E-126.57E-117.62E-111.69E-10 0.00E+0 0.00E+0
12 11
-6.96E-
HTP-nc [CTUh] 7.17E-8 2.59E-9 2.37E-9 2.60E-11 9.46E-9 0.00E+01.44E-10 4.57E-9 5.10E-9 1.42E-8 0.00E+0 0.00E+0 -2.38E-9
11
SQP [-] ND ND ND ND ND ND ND ND ND ND ND ND ND ND
PM = Potential incidence of disease due to PM emissions; IR = Potential Human exposure efficiency relative to U235; ETP-fw = Potential
Caption comparative Toxic Unit for ecosystems; HTP-c = Potential comparative Toxic Unit for humans (cancerogenic); HTP-nc = Potential
comparative Toxic Unit for humans (not cancerogenic); SQP = Potential soil quality index
The SQP indicator is not given due to considerable uncertainties in the calculation.
The result figures given in module B2 refer to a period of 1 year because a reference service life is not declared.
They have to be multiplied by the assumed service life (in years) of the floor covering in the building under
consideration.
Disclaimer 1 – for the indicator “Potential Human exposure efficiency relative to U235”.
This impact category deals mainly with the eventual impact of low dose ionizingradiation on human health of the
nuclear fuel cycle. It does not consider effects due to possible nuclear accidents, occupational exposure nor due
to radioactive waste disposal in undergroundfacilities. Potential ionizing radiation from the soil, from radon and
from some construction materials is also not measured by this indicator.
Disclaimer 2 – for the indicators “abiotic depletion potential for non-fossil resources”, “abiotic depletion potential
for fossil resources”, “water (user) deprivation potential, deprivation-weighted water consumption”, “potential
comparative toxic unit for ecosystems”, “potential comparative toxic unit for humans – cancerogenic”, “Potential
comparative toxic unit for humans - not cancerogenic”, “potential soil quality index”.
The results of this environmental impact indicator shall be used with care as the uncertainties on these results are
high or as there is limited experience with the indicator.
References
EN 1307 DIN EN ISO 14040:2006+A1:2020 Environmental
DIN EN 1307: 2014+A1:2016+A2:2018-05: Textile management - Life cycle assessment - Principles and
floor coverings - Classification framework
EN 13501-1 ISO 14044
DIN EN 13501-1:2019-05: Fire classification of DIN EN ISO 14044:2006+A1:2018+A2:2020
construction products and building elements - Part 1: Environmental management - Life cycle assessment -
Classification using data from reaction to fire tests Requirements and guidelines
EN 14041 ISO 15686
DIN EN 14041: 2018-05: Resilient, textile and laminate ISO 15686: Buildings and constructed assets -
floor coverings - Essential characteristics Service life planning
ISO 15686-1: 2011-05: Part 1: General principles and
EN 15804 framework
DIN EN 15804:2012+A2:2019 + AC:2021, ISO 15686-2: 2012-05: Part 2: Service life prediction
Sustainability of construction works — Environmental procedures
Product Declarations — Core rules for the product ISO 15686-7: 2017-04: Part 7: Performance
category of construction products evaluation for feedback of service life data
from practice
EN 16810 ISO 15686-8: 2008-06: Part 8: Reference service life
DIN EN 16810: 2017-08: Resilient, textile and laminate and service-life estimation
floor coverings – Environmental product declarations –
Product category rules Regulation (EU) No. 305/2011
Regulation No. 305/2011 Construction Products
ISO 10874 Regulation (CPR) of the European Council and of the
DIN EN ISO 10874: 2012+A1:2021-04: Resilient, European Parliament, April 2011
textile and laminate floor coverings - Classification
General Instructions for the IBU-EPD Program
ISO 14025 General Instructions for the EPD-Program of the
DIN EN /ISO 14025:2011-10/, Environmental labels Institut Bauen und Umwelt e.V., The Preparation of
and declarations — Type III environmental Environmental Product Declarations - EPDs, version
declarations — Principles and procedures 2.0, Institut Bauen und Umwelt e.V., Berlin, January
2021, www.ibu-epd.de
ISO 14040
7 Environmental Product Declaration Balsan – PILOTE 3D NRB - tufted carpet tiles
BNB, Nutzungsdauer von Bauteilen Part B: Requirements on the EPD for floor coverings,
Bewertungssystem Nachhaltiges Bauen (BNB), V1.2, Berlin: Institut Bauen und Umwelt e.V. (IBU),
Nutzungsdauer von Bauteilen, Bundesministerium des February 2018
Inneren, für Bau und Heimat, 24.02.2017
PRODIS
ECHA candidate list Product Information System (PRODIS) of the
Candidate List of substances of very high concern European Carpet Industry, Gemeinschaft
(SVHCs) for authorisation, 08.07.2021, European umweltfreundlicher Teppichboden e.V (GUT) and
Chemicals Agency (ECHA), Helsinki, Finland European Carpet and Rug Association
(ECRA), http://www.pro-dis.info
ecoinvent
ecoinvent, Zurich, Switzerland, database version 3.7, REACH
published September 2020 Regulation (EC) No 1907/2006 of the European
Parliament and of the Council of 18 December 2006
GaBi database concerning the Registration, Evaluation, Authorisation
GaBi Software-System and Database for Life Cycle and Restriction of Chemicals (REACH), June 2017,
Engineering, thinkstep AG, Leinfelden-Echterdingen, last update: 10.06.2022
2022-1
VDZ e.V.
PCR Part A Association of German Cement Works, Ed. Environ-
Product Category Rules for Building-Related Products mental Data of the German Cement Industry 2020
and Services Part A: Calculation Rules for the Life
Cycle Assessment and Requirements on the Project
Report according to EN 15804+A2:2019, V1.2, Berlin:
Institut Bauen und Umwelt e.V. (IBU), November 2021
PCR Part B
Product Category Rules for Building-Related Products
and Services
8 Environmental Product Declaration Balsan – PILOTE 3D NRB - tufted carpet tiles
Publisher
Institut Bauen und Umwelt e.V. Tel +49 (0)30 3087748- 0
Hegelplatz 1 Fax +49 (0)30 3087748- 29
10117 Berlin Mail info@ibu-epd.com
Germany Web www.ibu-epd.com
Programme holder
Institut Bauen und Umwelt e.V. Tel +49 (0)30 - 3087748- 0
Hegelplatz 1 Fax +49 (0)30 – 3087748 - 29
10117 Berlin Mail info@ibu-epd.com
Germany Web www.ibu-epd.com
Author of the Life Cycle
Assessment Tel +49 (0)241 96843 410
Gemeinschaft umweltfreundlicher Fax +49 (0)241 96843 400
Teppichboden (GUT) e.V. Mail mail@gut-ev.de
Schönebergstraße 2 Web www.gut-ev.org
52068 Aachen
Germany
Owner of the Declaration
Balsan Moquette Tel +33 (0) 254 2916 00
Corbilly 2 Fax +33 (0) 254 3679 08
36330 Arthon Mail cedric.charton@balsan.com
France Web www.balsan.com
