ENVIRONMENTAL PRODUCT DECLARATION
as per ISO 14025 and EN 15804+A2
Owner of the Declaration bauforumstahl e.V.
Publisher Institut Bauen und Umwelt e.V. (IBU)
Programme holder Institut Bauen und Umwelt e.V. (IBU)
Declaration number EPD-BFS-20230270-IBG1-EN
Issue date 06.10.2023
Valid to 05.10.2028
Structural Steel: Heavy Plates
bauforumstahl e.V.
www.ibu-epd.com | https://epd-online.com
1. General Information
bauforumstahl e.V. Structural Steel: Heavy Plates
Programme holder Owner of the declaration
IBU – Institut Bauen und Umwelt e.V. bauforumstahl e.V.
Hegelplatz 1 Sohnstraße 65
10117 Berlin 40237 Düsseldorf
Germany Germany
Declaration number Declared product / declared unit
EPD-BFS-20230270-IBG1-EN 1 metric ton of structural steel heavy plates
This declaration is based on the product category rules: Scope:
Structural steels, 01.08.2021 This environmental product declaration (EPD) covers structural steel heavy
(PCR checked and approved by the SVR) plates and refers to a specific product.
The Life Cycle Assessment is based on data collected from the following
plants of bauforumstahl e.V. member companies:
Issue date - Dillinger with the sites in Dillingen (Germany) and Dunkirk (France)
The data used represent >95 % of the annual production of heavy plates
06.10.2023
from bauforumstahl e.V. member companies.
The owner of the declaration shall be liable for the underlying information
and evidence; the IBU shall not be liable with respect to manufacturer
Valid to
information, life cycle assessment data and evidences.
05.10.2028
The EPD was created according to the specifications of EN 15804+A2. In
the following, the standard will be simplified as EN 15804.
Verification
The standard EN 15804 serves as the core PCR
Independent verification of the declaration and data according to ISO
14025:2011
internally X externally
Dipl.-Ing. Hans Peters
(Chairman of Institut Bauen und Umwelt e.V.)
Florian Pronold Dr.-Ing. Nikolay Minkov,
(Managing Director Institut Bauen und Umwelt e.V.) (Independent verifier)
1 Environmental Product Declaration - bauforumstahl e.V. - Structural Steel: Heavy Plates
2. Product
2.1 Product description/Product definition 2.4 Delivery status
This EPD refers to heavy plates, hot rolled products produced The dimensions of the declared products may vary according to
on dedicated quarto plate mills. The declaration covers various the intended application.
steel grades in various delivery conditions (grades S235 to
S960). The mean steel grades are structural steel grades, like 2.5 Base materials/Ancillary materials
low alloy structural steels, including weathering steels. Mean Structural steels are non-or low-alloy steel products whose
thickness value is at 20 mm but the declaration covers the carbon content is between 0 and 0.6 %. Iron is the main
whole range from 5 mm up to 510 mm. Width range is from component of steel plates. The content of other elements is
1000 mm up to 5200 mm. Weathering steels offer improved less than 2 %. The exact chemical composition varies
resistance to corrosion thanks to the addition of elements, like depending on the steel grade.
copper, chromium and nickel during manufacture. Additional
alloying elements can be added to increase the steel's tensile Auxiliary materials:
strength or make forming processes easier. For the placing of For the production route 'blast furnace with basic oxygen
the product on the market in the European Union/European furnace': coking coal, coal,
Free Trade Association lime, aluminium, ferroalloys (ferro silicon, ferro manganese,
(EU/EFTA) (with the exception of Switzerland) Regulation (EU) ferro nickel, ferro niobium, ferro vanadium, ferro titanium)
No. 305/2011 (CPR) applies. This product has a declaration of The rates of these additives depend on the steel grade.
performance taking into consideration EN 10025-1:2004 - Hot
rolled products of structural steels - Part 1: General technical The product for authorization contains substances on the
delivery conditions. For the application and use the respective ECHA list of substances of very high concern (SVHC) (14 July
national provisions apply. 2021) above 0.1 % by mass: No.
2.2 Application The product contains further carcinogenic, mutagenic,
Structural steels are intended for bolted, welded or otherwise reprotoxic (CMR) substances of category 1A or 1B that not in
connected constructions of buildings, bridges and other the candidate list, above 0.1 mass % in at least one
structures, or in composite steel and concrete structures. subproduct: No.
Examples are:
Biocides have been added to the construction product, or the
• single-storey buildings (industrial and storage halls, etc.)
product has been treated with biocides (a treated product
• multi-storey buildings (offices, residential buildings,
pursuant to the Biocidal Product Regulation (EU) No.
shops, car parks, high rise, etc.)
528/2012): No.
• bridges (railway bridge, road bridge, pedestrian bridge,
etc.)
2.6 Manufacture
• other structures (power plants, stadiums, convention
In the integrated steel production route iron ore, (typical mix
centres, airports, stations, etc.)
based on ferro-oxides Fe2O ) coke breeze, circulating
When weathering steel is exposed to the ambient atmosphere it 3
components and other additives are mixed and sintered in
develops an initial layer of iron oxide in the same way as
preparation for being fed into the blast furnace together with
carbon steel. The rate of oxidisation depends on how much
coking coke, which is the reducing agent. Also pellets and/or
oxygen, moisture, and atmospheric contaminants can access
lump may be used.
the surface of the metal. In the initial stages, a complex mix of
The pig iron produced in the blast furnace is transferred into the
iron oxides covers the surface to create a layer of rust. As the
basic oxygen furnace. In this vessel, the iron is converted into
process progresses, the rust layer forms a barrier against the
steel by lowering the carbon content of the iron by blowing
corrosive agents and the rate of corrosion slows.
oxygen into the melt (exothermic reaction). For temperature
2.3 Technical Data control, steel scrap (up to 35 %) is added to the melt.
This EPD is valid for plates of varied grades and different forms
of delivery. Specific information on dimension tolerances, At the end of the steelmaking process, the liquid steel is mainly
constructional data, as well as mechanical and chemical transformed into a semi-finished product in a continuous
properties can be found in the relevant literature and/or the casting machine.
standards. The semi-product (slab) is hot-rolled into the final product
dimensions (heavy plate)
Constructional data
Name Value Unit Quality control: ISO 9001 Monitoring according to the product
Density 7850 kg/m3 standards, e.g. EN 10025, Part 1.
Modulus of elasticity 210000 N/mm2
2.7 Environment and health during manufacturing
Coefficient of thermal expansion 12 10-6K-1 No measures relating to safety, health and environmental
Thermal conductivity at 20°C λ 48 W/(mK) protection during the manufacturing process extending beyond
Melting point depending on the alloy national guidelines are required.
1536 °C
proportions up to
2.8 Product processing/Installation
Shear modulus 81000 N/mm2
Processing recommendations:
Performance data of the product in accordance with the Planning, processing, implementation and intended use of
declaration of performance with respect to its essential section and plate constructions have
characteristics according to EN 10025, Hot rolled products of to be carried out depending on the respective applications
structural steels. Further product standards can be: EN 10225, according to the generally recognized rules of engineering and
ASTM A36, A572, A514, A709 and A1066. manufacturer's recommendations. The standards of EN 1993
2 Environmental Product Declaration - bauforumstahl e.V. - Structural Steel: Heavy Plates
and EN 1994 (EUROCODE EC3 and EC4) apply to the design painting. At the end of life, weathering steel products are
of steel structures and composite steel and concrete structures. recovered, reused or recycled as well. The purpose, possible
They include the requirements regarding serviceability, bearing corrosion protection and adequate maintenance are decisive
capacity, durability and fire for service life.
resistance of steel structures EC3 and composite steel and
concrete structures EC4. 2.13 Extraordinary effects
The Standard Parts 1+2 of EN 1090 apply to the execution of Fire
steel structures and include the requirements for factory The material is class A1, i.e. not flammable per EN 13501.
production control. The material does not emit fumes or fire-gases.
In addition, the European Standards will work in connection Fire safety
with national amendments, national instructions, guidelines and
Name Value
publications, as well as legal provisions.
Building material class acc. EN 13501-1 A1
Regarding transport and storage of heavy plates, the generally
accepted requirements for securing loads have to be observed.
Instruction details of the manufacturer based on verified Water
standards and guidelines regarding welding, galvanizing as well Steel is stable to water, insoluble and does not emit substances
as hot and cold forming are to be observed in every case. in water. In case of flooding, no impacts are to be expected.
Steel can corrode in the presence of oxygen in the water (=
Occupational safety / Environmental protection: slow oxidation).
When processing/using steel plates according to the generally
recognized rules of engineering there are no measures to be Mechanical destruction
taken which are going beyond the public occupational health Due to the ductility of steel, steel structures react resilient in the
and safety. event of unforeseeable mechanical destruction: In case of
The processing/using of steel plates pursuant to the generally tensile load necking will occur before cracking. In case of a
recognized rules of engineering does not release substantial lasting high compression load, components of steel may buckle
environmental pollutants. Particular measures to protect the or bulge. No splintering or breaking edges shall result.
environment are not required.
2.14 Re-use phase
Residual material: General:
During processing residual pieces as well as turnings are to be After the service life of structural steel constructions the
separately collected. This scrap steel is entirely recycled by material is collected as secondary material for
melting and producing new steel products. recycling or reuse.
Recycling:
2.9 Packaging Structural steel is 100 % recyclable to new products of similar
Structural steels are delivered unpacked. or higher quality. Due to the magnetic properties, even small
amounts are regained after dismantling. Possible coatings
2.10 Condition of use
(metallic, organic or intumescent) do not limit the recyclability.
Structural steels are non-/low-alloyed steel products generated On the European market 88 % of the products are used for
by alloying iron with other metals and non-metals (esp. carbon). closed-loop recycling.
Iron is the main component of steel plates. The components are Reuse:
listed under chapter 2.5 'Base materials'. During usage, no Structural steel elements can be reused. On the European
changes in material composition shall occur. market 11 % of the products are reused after dismantling. Data
from industry estimates based on the following sources:
2.11 Environment and health during use
European Commission Technical Steel Research
The intended use of steel plates does not pose a hazard to
health or the environment in any known way. 2.15 Disposal
Due to its high value, steel scrap is not disposed, but fed into a
2.12 Reference service life
well-established endless cycle of reuse and recycling. However,
A reference service life for heavy steel plates is not declared.
in case of dumping due to collection loss no environmental
Heavy steel plates are construction products with many
impacts are expected.
different application purposes. The lifetime therefore will be
Waste code according to European Waste Catalogue EWC: 17
limited by the application as well as the service life of the work.
04 05 - iron and steel
Bridges using heavy plates are designed and calculated
according to Eurocodes to ensure more than 100 years of 2.16 Further information
durability. First structural steel projects using weathering steel Additional information on constructing with steel can be
were completed 50 years ago in Europe and have obtained from www.bauforumstahl.de.
demonstrated a very low maintenance level and no need for
3. LCA: Calculation rules
Name Value Unit
3.1 Declared Unit
Declared unit 1 t
The reference unit is 1 ton of structural steel heavy plates.
Density 7850 kg/m3
Foreground data describing the on-site production are Conversion factor to 1 kg 0.001 -
integrated into the LCA FE Software model for all sites under
The EPD is representative for all steel products covered by the
study. The LCI is assessed based on annual production data.
declared unit.
Background data are taken from the LCA FE Database.
Declared unit 3.2 System boundary
3 Environmental Product Declaration - bauforumstahl e.V. - Structural Steel: Heavy Plates
Type of the EPD: cradle-to-gate - with options: Modules A1-A3, Technological: All primary and secondary data are modelled to
Modules C1-C4 and Module D were considered. be specific to the technologies or technology mixes under
study. Where technology-specific data are unavailable, proxy
Modules A1-A3 cover the production stage including the data are used. The overall technological representativeness is
upstream burdens of purchased raw materials (iron ore, ferro- considered to be good.
alloys, lime, dolomite, etc.), their transports and the integrated
steel production at the production site under study. Material and Geographical: All primary and secondary data are collected
energy flows for coke making, the sinter plant, the blast specific to the country /region under study. Where
furnace, the basic oxygen furnace and the hot strip mills are country/region-specific data are unavailable, proxy data are
considered. used. The overall geographical representativeness is
considered to be good.
Modules C1-C4 consider the dismantling of the considered
product (C1), the transportation of the dismantled components Temporal: All primary data are collected for a representative
to their final EoL destination (C2), the waste processing for year (2021). All secondary data come from the Sphera LCA FE
reuse, recovery or recycling (C3) as well as the disposal (C4). Databases and are representative of the years 2017-2022. As
the study intended to compare the product systems for the
Module D refers to the End-of-Life, including recycling and/or reference year 2021, temporal representativeness is good.
reuse.
3.7 Period under review
3.3 Estimates and assumptions The foreground data collected by the manufacturer are based
All assumptions are documented in detail and represent the on yearly production amounts and refer to 2021.
reality best possible based on available data.
Due to lack of available datasets for some alloying elements 3.8 Geographic Representativeness
(e.g. ferro vanadium) South-African datasets were used instead Land or region, in which the declared product system is
of local data. The use of South-African data sets represents a manufactured, used or handled at the end of the product´s
'worst case' assumption for European production so the set-up lifespan: Western Europe
scenario is considered conservative approach. Based on the
LCA practitioner's knowledge working with the respective
3.9 Allocation
industries, the proxy for silico-manganese was considered as
75 % ferro manganese and 25 % ferro silicon. Primary data are allocated using the partitioning approach
developed by worldsteel/EUROFER for calculating life cycle
3.4 Cut-off criteria inventories of co-products in steel production. The so-called
No cut-off criteria are applied in this study. All reported data coproduct methodology allocates environmental effects to the
were incorporated and modelled using the best available LCI steelmaking process and the emerging co-products based on
data. physical relations. Material-inherent flow properties are thus
Packaging materials and their transportation, or the steel straps taken into account.
used to bundle the considered steel products for delivery, are
3.10 Comparability
neglected due to low contribution to the overall life cycle
results. Basically, a comparison or an evaluation of EPD data is only
possible if all the data sets to be compared were created
3.5 Background data according to EN 15804 and the building context, respectively
Secondary data from the LCA FE Database (former GaBi) were the product-specific characteristics of performance, are taken
used to model the background system in the LCA model. into account. The LCA FE Database (CUP version 2022.2) was
used to calculate the LCA.
3.6 Data quality
4. LCA: Scenarios and additional technical information
Re-use, recovery- and recycling potential (D)
Characteristic product properties of biogenic carbon
The declared product does not include biogenic carbon. Name Value Unit
Recycling - Scenario 1 1000 kg
End-of-Life Scenarios Recycling - Scenario 2 0 kg
The EPD covers three End-of-Life scenarios
Recycling - Scenario 3 880 kg
(SteelConstruction-info; European Commission Technical Steel
Reuse - Scenario 1 0 kg
Research):
Reuse - Scenario 2 1000 kg
• Scenario 1: 100 % Recycling
Reuse - Scenario 3 110 kg
• Scenario 2: 100 % Reuse
• Scenario 3: European average 88 % Recycling, 11 %
Reuse and 1 % Loss
End of life (C1-C4)
Name Value Unit
Landfilling - Scenario 1 0 kg
Landfilling - Scenario 2 0 kg
Landfilling - Scenario 3 10 kg
4 Environmental Product Declaration - bauforumstahl e.V. - Structural Steel: Heavy Plates
5. LCA: Results
The following table contains the LCA results for a declared unit of 1 ton structural steel heavy plates.
DESCRIPTION OF THE SYSTEM BOUNDARY (X = INCLUDED IN LCA; ND = MODULE OR INDICATOR NOT DECLARED; MNR =
MODULE NOT RELEVANT)
Benefits and
Construction loads beyond
Product stage Use stage End of life stage
process stage the system
boundaries
la ire ta m w a Ry lp p u s tro p s n a rT g n iru tc a fu n a M e h t m o rf tro p s n a rTe tis e h t o t e ta g y lb m e s s A e s U e c n a n e tn ia M ria p e R tn e m e c a lp e R tn e m h s ib ru fe R y g re n e la n o ita re p Oe s u re ta w la n o ita re p Oe s u n o itc u rts n o c -e Dn o itilo m e d tro p s n a rT g n is s e c o rp e ts a W la s o p s iD -e s u e R-y re v o c e R-g n ilc y c e Rla itn e to p
A1 A2 A3 A4 A5 B1 B2 B3 B4 B5 B6 B7 C1 C2 C3 C4 D
X X X MND MND MND MND MNR MNR MNR MND MND X X X X X
RESULTS OF THE LCA - ENVIRONMENTAL IMPACT according to EN 15804+A2: 1 ton structural steel
Parameter Unit A1-A3 C1 C2 C3/1 C3/2 C3/3 C4/1 C4/2 C4/3 D/1 D/2 D/3
GWP-total kg CO 2 eq 2.53E+03 2.19E+00 2.51E+00 0 0 0 0 0 1.45E-01 -1.36E+03 -2.53E+03 -1.47E+03
GWP-fossil kg CO 2 eq 2.53E+03 2.86E+00 2.52E+00 0 0 0 0 0 1.49E-01 -1.36E+03 -2.53E+03 -1.47E+03
GWP-
biogenic kg CO 2 eq 4.03E-01 -7.61E-01 -2.47E-02 0 0 0 0 0 -4.42E-03 6.93E-01 -4.08E-01 5.63E-01
GWP-luluc kg CO 2 eq 9.07E-01 9.32E-02 1.7E-02 0 0 0 0 0 2.75E-04 -2.8E-02 -9.03E-01 -1.24E-01
kg CFC11
ODP 5.5E-10 5.72E-12 2.48E-13 0 0 0 0 0 3.51E-13 -2.97E-12 -5.5E-10 -6.31E-11
eq
AP mol H+ eq 5.37E+00 1.1E-02 2.65E-03 0 0 0 0 0 1.06E-03 -2.91E+00 -5.37E+00 -3.15E+00
EP-
kg P eq 1.1E-03 5.1E-05 9.03E-06 0 0 0 0 0 2.53E-07 -2.46E-04 -1.09E-03 -3.36E-04
freshwater
EP-marine kg N eq 1.33E+00 2.17E-03 8.17E-04 0 0 0 0 0 2.71E-04 -5.12E-01 -1.33E+00 -5.95E-01
EP-terrestrial mol N eq 1.45E+01 2.83E-02 9.87E-03 0 0 0 0 0 2.97E-03 -4.5E+00 -1.45E+01 -5.54E+00
kg NMVOC
POCP 5.67E+00 8.5E-03 2.25E-03 0 0 0 0 0 8.22E-04 -2.08E+00 -5.67E+00 -2.45E+00
eq
ADPE kg Sb eq 3.63E-03 1.52E-06 2.55E-07 0 0 0 0 0 1.53E-08 -3.38E-03 -3.63E-03 -3.36E-03
ADPF MJ 2.4E+04 2.4E+02 3.32E+01 0 0 0 0 0 1.95E+00 -1.25E+04 -2.4E+04 -1.36E+04
m3 world eq
WDP 1.4E+02 2.3E-01 2.83E-02 0 0 0 0 0 1.64E-02 -2.52E+02 -1.4E+02 -2.36E+02
deprived
GWP = Global warming potential; ODP = Depletion potential of the stratospheric ozone layer; AP = Acidification potential of land and water; EP =
Eutrophication potential; POCP = Formation potential of tropospheric ozone photochemical oxidants; ADPE = Abiotic depletion potential for non-fossil
resources; ADPF = Abiotic depletion potential for fossil resources; WDP = Water (user) deprivation potential)
RESULTS OF THE LCA - INDICATORS TO DESCRIBE RESOURCE USE according to EN 15804+A2: 1 ton structural steel
Parameter Unit A1-A3 C1 C2 C3/1 C3/2 C3/3 C4/1 C4/2 C4/3 D/1 D/2 D/3
PERE MJ 8.26E+02 1.6E+01 2.3E+00 0 0 0 0 0 2.93E-01 7.85E+02 -8.25E+02 5.98E+02
PERM MJ 0 0 0 0 0 0 0 0 0 0 0 0
PERT MJ 8.26E+02 1.6E+01 2.3E+00 0 0 0 0 0 2.93E-01 7.85E+02 -8.25E+02 5.98E+02
PENRE MJ 2.4E+04 2.41E+02 3.33E+01 0 0 0 0 0 1.96E+00 -1.25E+04 -2.4E+04 -1.36E+04
PENRM MJ 0 0 0 0 0 0 0 0 0 0 0 0
PENRT MJ 2.4E+04 2.41E+02 3.33E+01 0 0 0 0 0 1.96E+00 -1.25E+04 -2.4E+04 -1.36E+04
SM kg 2.17E+02 0 0 0 0 0 0 0 0 0 0 0
RSF MJ 0 0 0 0 0 0 0 0 0 0 0 0
NRSF MJ 0 0 0 0 0 0 0 0 0 0 0 0
FW m3 4.68E+00 1.76E-02 2.66E-03 0 0 0 0 0 4.97E-04 -5.69E+00 -4.68E+00 -5.51E+00
PERE = Use of renewable primary energy excluding renewable primary energy resources used as raw materials; PERM = Use of renewable primary
energy resources used as raw materials; PERT = Total use of renewable primary energy resources; PENRE = Use of non-renewable primary energy
excluding non-renewable primary energy resources used as raw materials; PENRM = Use of non-renewable primary energy resources used as raw
materials; PENRT = Total use of non-renewable primary energy resources; SM = Use of secondary material; RSF = Use of renewable secondary fuels;
NRSF = Use of non-renewable secondary fuels; FW = Use of net fresh water
RESULTS OF THE LCA – WASTE CATEGORIES AND OUTPUT FLOWS according to EN 15804+A2:
1 ton structural steel
Parameter Unit A1-A3 C1 C2 C3/1 C3/2 C3/3 C4/1 C4/2 C4/3 D/1 D/2 D/3
HWD kg 3.17E-07 1.62E-09 1.76E-10 0 0 0 0 0 1E-10 -9.62E-08 -3.17E-07 -1.19E-07
NHWD kg 5.3E+00 3.75E-02 5.43E-03 0 0 0 0 0 1E+01 1.89E+02 -5.3E+00 1.65E+02
RWD kg 1.88E-01 1.21E-03 6.18E-05 0 0 0 0 0 2.17E-05 1.55E-03 -1.88E-01 -1.94E-02
CRU kg 0 0 0 0 1E+03 1.1E+02 0 0 0 0 0 0
MFR kg 0 0 0 1E+03 0 8.8E+02 0 0 0 0 0 0
5 Environmental Product Declaration - bauforumstahl e.V. - Structural Steel: Heavy Plates
MER kg 0 0 0 0 0 0 0 0 0 0 0 0
EEE MJ 0 0 0 0 0 0 0 0 0 0 0 0
EET MJ 0 0 0 0 0 0 0 0 0 0 0 0
HWD = Hazardous waste disposed; NHWD = Non-hazardous waste disposed; RWD = Radioactive waste disposed; CRU = Components for re-use;
MFR = Materials for recycling; MER = Materials for energy recovery; EEE = Exported electrical energy; EET = Exported thermal energy
RESULTS OF THE LCA – additional impact categories according to EN 15804+A2-optional:
1 ton structural steel
Parameter Unit A1-A3 C1 C2 C3/1 C3/2 C3/3 C4/1 C4/2 C4/3 D/1 D/2 D/3
Disease
PM ND ND ND ND ND ND ND ND ND ND ND ND
incidence
kBq U235
IR ND ND ND ND ND ND ND ND ND ND ND ND
eq
ETP-fw CTUe ND ND ND ND ND ND ND ND ND ND ND ND
HTP-c CTUh ND ND ND ND ND ND ND ND ND ND ND ND
HTP-nc CTUh ND ND ND ND ND ND ND ND ND ND ND ND
SQP SQP ND ND ND ND ND ND ND ND ND ND ND ND
PM = Potential incidence of disease due to PM emissions; IR = Potential Human exposure efficiency relative to U235; ETP-fw = Potential comparative
Toxic Unit for ecosystems; HTP-c = Potential comparative Toxic Unit for humans (cancerogenic); HTP-nc = Potential comparative Toxic Unit for humans
(not cancerogenic); SQP = Potential soil quality index
The additional and optional impact categories according to EN15804+A2 are not declared as this is not required according to PCR Part
A.
Disclaimer 1 – for the indicator 'Potential Human exposure efficiency relative to U235'. This impact category deals mainly with the
eventual impact of low-dose ionizing radiation on human health of the nuclear fuel cycle. It does not consider effects due to possible
nuclear accidents, occupational exposure or radioactive waste disposal in underground facilities. Potential ionizing radiation from the
soil, radon and from some construction materials is also not measured by this indicator.
Disclaimer 2 – for the indicators 'abiotic depletion potential for non-fossil resources', 'abiotic depletion potential for fossil resources',
'water (user) deprivation potential, deprivation-weighted water consumption', 'potential comparative toxic unit for ecosystems', 'potential
comparative toxic unit for humans – cancerogenic', 'Potential comparative toxic unit for humans - not cancerogenic', 'potential soil
quality index'. The results of this environmental impact indicator shall be used with care as the uncertainties on these results are high
as there is limited experienced with the indicator.
6. LCA: Interpretation
The following figure shows the results of the individual modules
for all considered End-of-Life scenarios using the example of
climate change.
considered scenarios and varies significantly depending on the
It is visible that module D represents a credit within all considered End-of-Life scenario. The manufacturing phase
6 Environmental Product Declaration - bauforumstahl e.V. - Structural Steel: Heavy Plates
(module A1-3) dominates the product system for all scenarios.
The following tables give a detailed evaluation of all LCIA
results of the production phase (A1-A3):
As can be seen from the table, direct process emissions of consumed in the basic oxygen furnace, natural gas consumed
steel production (coke making, sinter plant, blast furnace, basic within most of the on-site processes) dominate the
oxygen furnace, hot rolling, and boiler/on-site power plant) and environmental effects across all selected impact categories.
the supply chain of purchased raw materials and energy The environmental impact of the products correlates directly
carriers (e.g. coal for coke making, pellet feed and iron ore with their mass.
consumed within the sinter plant and blast furnace, ferro-alloys
7. Requisite evidence
This EPD covers semi-finished structural steel of hot rolled atmosphere (corrosivity categories according to EN ISO 12944-
construction products. Further processing and fabrication 2.
depend on the intended application. Therefore, further If required, the surfaces of fabricated structural components are
documentation is not applicable. 7.1 Weathering performance usually protected with anticorrosion material in order to prevent
The rusting rate of unalloyed steel depends on the position of any direct contact with the atmosphere. The weathering of this
the component and the conditions of the surrounding protection depends on the applied protection system.
8. References
CPR LCA for Experts Software System and Database for Life Cycle
Regulation (EU) No 305/2011 of the European Parliament and Engineering, Sphera Solution GmbH, Leinfelden-Echterdingen,
of the Council of 9 March 2011 laying down harmonised CUP Version 2022.2 (https://www.gabi-
conditions for the marketing of construction products and software.com/support/gabi)
repealing Council Directive 89/106/EEC Text with EEA
relevance PCR, Part A
Product Category Rules for Building-Related Products and
European Commission Technical Steel Research Services, Calculation Rules for the Life Cycle Assessment and
Sansom, M. and Meijer, J.: Life-cycle assessment (LCA) for Requirements on the Project Report. Institut Bauen und Umwelt
steel construction, European Commission technical steel e.V. (IBU), version 1.3, 2021, www.bau-umwelt.de
research, 2001-12
PCR, Part B
EWC Requirements on the EPD for Structural steels, 01/08/2021
European Waste Catalogue (PCR checked and approved by the SVR) – Institut Bauen und
Umwelt e.V. (IBU), Königswinter
German Ministry of Environmental Affairs
"Instrumente zur Wiederverwendung von Bauteilen und SteelConstruction-info
hochwertigen Verwertung von Baustoffen" https://www.steelconstruction.info/The_recycling_and_reuse_survey
LCA FE Software / Database worldsteel/EUROFER
7 Environmental Product Declaration - bauforumstahl e.V. - Structural Steel: Heavy Plates
Bollen, J., Avery N., Millar, I. and Broadbent, C.: Methodology to EN 1993:2010-12/ Eurocode 3
determine the LCI of steel industry co-products, 2013 Design of steel structures
Standards
EN 1994:2010-12 / Eurocode 4
AISC 303-10 Design of composite steel and concrete structures
Code of Standard Practice for Steel Buildings and Bridges
EN 10025:2005-2
ANSI/AISC 360-16 Hot rolled products of structural steels
Specification for Structural Steel Buildings
EN 10225
Weldable structural steels for fixed offshore structures
ASTM A 36-14
Standard specification for carbon structural steel EN 13501:2010-1
Fire classification of construction products and building
ASTM A514-14 elements
Standard Specification for High-Yield-Strength, Quenched and
Tempered Alloy Steel Plate, Suitable for Welding EN 15804
EN 15804:2019+A2, Sustainability of construction works —
ASTM A572-15 Environmental Product Declarations — Core rules for
Standard Specification for High-Strength Low-Alloy Columbium- theproduct category of construction products
Vanadium Structural Stee
ISO 9001:2015
ASTM A709-13 Quality management systems - Requirements
Standard Specification for Structural Steel for Bridges
ISO 12944-2:2017-11
ASTM A1066-11(15) Paints and varnishes - Corrosion protection of steel structures
Standard Specification for High-Strength Low-Alloy Structural by protective paint systems - Part 2: Classification of
Steel Plate Produced by environments
Thermo-Mechanical Controlled Process (TMCP)
ISO 14001:2015
AWS D1.1/D1.1M-15 Environmental management systems - Requirements with
Structural Welding Code – Steel guidance for use
EN 1090:2018 ISO 14025
Execution of steel structures and aluminium structures Environmental labels and declarations — Type III
environmental declarations —Principles and procedures
8 Environmental Product Declaration - bauforumstahl e.V. - Structural Steel: Heavy Plates
Publisher
Institut Bauen und Umwelt e.V. +49 (0)30 3087748- 0
Hegelplatz 1 info@ibu-epd.com
10117 Berlin www.ibu-epd.com
Germany
Programme holder
Institut Bauen und Umwelt e.V. +49 (0)30 3087748- 0
Hegelplatz 1 info@ibu-epd.com
10117 Berlin www.ibu-epd.com
Germany
Author of the Life Cycle Assessment
Sphera Solutions GmbH +49 (0)711 341817-0
Hauptstraße 111- 113 info@sphera.com
70771 Leinfelden-Echterdingen www.sphera.com
Germany
Owner of the Declaration
bauforumstahl e.V. 0211-54012080
Sohnstraße 65 zentrale@bauforumstahl.de
40237 Düsseldorf www.bauforumstahl.de
Germany
Dillinger +49 6831 470
Werkstraße 1 info@dillinger.biz
66763 Dillingen/Saar www.dillinger.de
Germany
9 Environmental Product Declaration - bauforumstahl e.V. - Structural Steel: Heavy Plates
