ENVIRONMENTAL PRODUCT DECLARATION
as per ISO 14025 and EN 15804+A2
Owner of the Declaration Mostostal Siedlce Limited liability company LP
Programme holder Institut Bauen und Umwelt e.V. (IBU)
Publisher Institut Bauen und Umwelt e.V. (IBU)
Declaration number EPD-MOS-20220213-CBA1-EN
Issue date 16.11.2022
Valid to 15.11.2027
Steel structures, pallets and platform gratings
+ coating (optional)
Mostostal Siedlce
Limited liability company LP
www.ibu-epd.com | https://epd-online.com
Umwelt Produktdeklaration Name des Herstellers – Name des Produkts
General Information
Mostostal Siedlce Steel structures, pallets and
Limited liability company LP platform gratings + coating
(optional)
Programme holder Owner of the declaration
IBU – Institut Bauen und Umwelt e.V. Mostostal Siedlce Limited liability company LP
Hegelplatz 1 Terespolska 12
10117 Berlin 08-110 Siedlce
Germany Poland
Declaration number Declared product / declared unit
EPD-MOS-20220213-CBA1-EN 1 ton of representative steel structure, pallets or
platform gratings
This declaration is based on the product Scope:
category rules: Steel alloy is the main material, used in over 98% of
Structural steels, 11.2017 production and it was modelled as the mean value on
(PCR checked and approved by the SVR) the basis of the safety data sheets purchased steel
received from the company.
Issue date
16.11.2022 EPD covered: galvanized structures, painted
structures, duplex structures, structures without
protection, galvanized pallets, galvanized gratings, and
Valid to
gratings without protection.
15.11.2027
The owner of the declaration shall be liable for the
underlying information and evidence; the IBU shall not
be liable with respect to manufacturer information, life
cycle assessment data and evidences.
The EPD was created according to the specifications
of EN 15804+A2. In the following, the standard will be
simplified as EN 15804.
Verification
The standard EN 15804 serves as the core PCR
Independent verification of the declaration and data
according to ISO 14025:2011
Dipl. Ing. Hans Peters internally x externally
(chairman of Institut Bauen und Umwelt e.V.)
Dr. Alexander Röder Vito D'Incognito
(Managing Director Institut Bauen und Umwelt e.V.)) (Independent verifier)
Product
Product description/Product definition Application
The analyzed products include steel structures, The products covered in the EPD:
platform gratings and pallets. In addition, they may be  Galvanized structures;
covered with anti-corrosion protection, which is applied  Painted structures;
using hot galvanizing according to EN ISO 1461 (DIN
 Duplex structures;
50976), painting or power painting in a range of
 Structures without protection;
colours.
 Galvanized pallets;
For the placing on the market of the product in the  Galvanized gratings;
European Union/European Free Trade Association
 Gratings without protection.
(EU/EFTA) (with the exception of Switzerland)
Regulation EU No. 305/2011 (CPR) applies. The
product needs a declaration of performance taking into
consideration EN 1090-1 and the CE-marking. For the Technical Data
application and use the respective national provisions Mostostal Siedlce manufactures steel structures based
apply. on the technical documentation of the customer and
based on the internal documentation, developed by
constructors working at the Company. Documentation
2 Environmental Product Declaration Mostostal – Steel structures, pallets and platform gratings + coating (optional)
is developed according to the standards: PN, DIN, EN,
EUROCODES and GOST in the following languages:
Polish, Russian, German and English. Used IT tools Performance data of the product in accordance with
are: Robot, Staad-Pro, Microstation– Structural, Rm- the declaration of performance with respect to its
win, ABCpłyta, MathCad, Tekla, Bocad, RCad, and essential characteristics according to EN 1090-2.
Autocad. The maximum dimensions for indivisible
components composing a product are as follows: L = Base materials/Ancillary materials
30 m, B = 6.3 m, H = 4.2 m and correspond to the Structural steels are non-or low-alloy steel products
weight of 64 tonnes. Steel structures are carried out whose carbon content is amount 0.16%, Mn - 1,3%, Si
according to the standards: EN 1090-1-2, BSK 07, DIN 0.17%, Cr 0,04%, Ni 0.04%., Cu 0.10%, Mo, 0.01%.
18800-7, DIN 15018, DS 804, DIN 19704, AWS D1.1. Iron is the main component of steel.
Platform gratings are manufactured in accordance with Abrasive blasting (shot peening) and chemical
DIN 24537. treatment (etching in acids) is employed.
The metallic coating according EN 10346:
Constructional data Zn<99.995%
Name Value Unit Painting protection: using the hydrodynamic method.
Density 7850 kg/m3
EN 1090- This product/article/at least one partial article contains
Tolerances on dimension and
2; Annex substances listed in the candidate list (date:
shape
B, Class 2 09.09.2022) exceeding 0.1 percentage by mass: no.
EN 10025-
Weldability 2; EN Reference service life
10219 not applicable
Facture tougheness/brittle
27 J
strength 20 degrees Celsius
Reaction to fire A1 Class
EN ISO
Durability / Corrosion protection 1461; EN
ISO 12944
LCA: Calculation rules
Declared Unit A1-A3: Manufacturing of pre-products, packaging,
This declaration applies to 1 ton of analysed products ancillary materials, transport to the factory, production
(steel structures, pallets and platform gratings). including energy supply and waste handling,
The LCA is calculated based on averaged volume A4: Transport to building site,
production data of the contributing plants. C1:Deconstruction, demolition,
C2:Transport to waste processing plant,
Declared unit C3:Waste processing,
Name Value Unit C4: Waste disposal (incineration).
Declared unit 1 t D: Potential for reuse, recovery and/or recycling
(benefits for incineration and recovery of packaging
Type of EPD: Declaration of a representative product materials from module A5 and envelopes incineration
from the manufacturer´s plants. from module C4).
System boundary Comparability
Type of EPD: Cradle-to-gate (with options) Basically, a comparison or an evaluation of EPD data
The system boundaries of the EPD follow the modular is only possible if all the data sets to be compared
construction system as described by EN 15804. were created according to EN 15804 and the building
The LCA takes into account the following modules: context, respectively the product-specific
characteristics of performance, are taken into account.
SimaPro software and databases (mainly Ecoinvent)
were used as a calculation basis.
LCA: Scenarios and additional technical information
Characteristic product properties
Information on biogenic Carbon
. An average of around 85% of all steel is recycled at
the end of a product’s life. These values are based on
Information on describing the biogenic Carbon expert judgement amongst the worldsteel LCA experts
Content at factory gate in 2020 (WSA). 15% of the end of life of steel was
Name Value Unit modelled as landfill.
Biogenic Carbon Content in
- kg C
product
Biogenic Carbon Content in .
1263.99 kg C
accompanying packaging
3 Environmental Product Declaration Mostostal – Steel structures, pallets and platform gratings + coating (optional)
End of life (C1 - C4)
50% is cutting the dismantled structures with electricity
and 50% is cutting the dismantled structures with
welding gas.
25 m of cutting is needed for 1 ton of structures,
gratings and pallets.
Transport of used products and packaging: 100 km.
Name Value Unit
Collected separately : packaging
2581 kg
materials
Collected as mixed construction
150 kg
waste : steel
Energy recovery 1290 kg
Landfilling 1440 kg
Reuse, recovery and/or recycling potentials (D),
relevant scenario information
The avoided production of primary steel sheet is
considered. Resulting potential benefits and loads for
metal recycling are declared in module D.
4 Environmental Product Declaration Mostostal – Steel structures, pallets and platform gratings + coating (optional)
LCA: Results
.
DESCRIPTION OF THE SYSTEM BOUNDARY (X = INCLUDED IN LCA; ND = MODULE OR INDICATOR NOT
DECLARED; MNR = MODULE NOT RELEVANT)
BENEFITS AND
CONSTRUCTI LOADS
PRODUCT STAGE ON PROCESS USE STAGE END OF LIFE STAGE BEYOND THE
STAGE SYSTEM
BOUNDARIES
5 Environmental Product Declaration Mostostal – Steel structures, pallets and platform gratings + coating (optional)
lairetam
waR
ylppus tropsnarT
gnirutcafunaM
eht
morf
tropsnarT
etis
eht
ot
etag
ylbmessA esU
ecnanetniaM
riapeR
tnemecalpeR tnemhsibrufeR
ygrene
lanoitarepO esu
retaw
lanoitarepO esu
noitcurtsnoc-eD
noitilomed tropsnarT
gnissecorp
etsaW
lasopsiD -esueR -yrevoceR -gnilcyceR laitnetop
A1 A2 A3 A4 A5 B1 B2 B3 B4 B5 B6 B7 C1 C2 C3 C4 D
X X X X ND ND ND MNR MNR MNR ND ND X X X X X
RESULTS OF THE LCA - ENVIRONMENTAL IMPACT according to EN 15804+A2: declared unit and
product
Core Indicator Unit A1 A2 A3 A4 C1 C2 C3 C4 D
GWP-total [kg CO2-Eq.] 1.74E+3 1.97E+2 2.10E+3 9.72E+1 5.62E+0 3.19E+1 1.28E+1 1.23E+2 -4.63E+2
GWP-fossil [kg CO2-Eq.] 1.73E+3 1.97E+2 2.09E+3 9.71E+1 5.60E+0 3.18E+1 1.28E+1 2.19E+1 -4.63E+2
GWP-biogenic [kg CO2-Eq.] 2.66E+0 6.53E-2 2.55E+0 3.00E-2 1.55E-2 1.10E-2 1.92E-2 1.01E+2 -1.11E-1
GWP-luluc [kg CO2-Eq.] 1.02E+0 6.32E-2 5.12E+0 2.42E-2 9.58E-3 9.04E-3 7.29E-3 4.10E-3 -5.97E-2
ODP [kg CFC11-Eq.] 9.08E-5 4.53E-5 1.58E-4 2.29E-5 2.05E-7 7.62E-6 2.26E-6 2.15E-6 -2.02E-5
AP [mol H+-Eq.] 8.52E+0 7.15E-1 1.25E+1 7.49E-1 2.53E-2 1.22E-1 1.10E-1 2.59E-1 -1.63E+0
EP-freshwater [kg P-Eq.] 9.90E-2 1.43E-3 1.07E-1 6.28E-4 3.06E-4 2.33E-4 3.79E-4 2.56E-4 -2.31E-2
EP-marine [kg N-Eq.] 1.72E+0 1.99E-1 1.97E+0 1.97E-1 4.59E-3 3.48E-2 4.29E-2 1.60E-1 -3.67E-1
EP-terrestrial [mol N-Eq.] 1.90E+1 2.20E+0 2.04E+1 2.18E+0 4.83E-2 3.85E-1 4.72E-1 1.32E+0 -3.97E+0
POCP [kg NMVOC-Eq.] 8.18E+0 7.10E-1 1.05E+1 6.38E-1 1.51E-2 1.29E-1 1.28E-1 3.57E-1 -2.24E+0
ADPE [kg Sb-Eq.] 1.11E-1 6.53E-4 5.30E-3 2.03E-4 1.13E-5 7.60E-5 6.04E-7 4.19E-6 -4.41E-5
ADPF [MJ] 1.90E+4 3.01E+3 2.32E+4 1.51E+3 6.95E+1 5.06E+2 2.02E+2 2.10E+2 -4.69E+3
[m³ world-Eq
WDP 5.71E+2 8.65E+0 1.66E+1 4.41E+0 1.89E+0 1.67E+0 7.24E-1 -1.62E+1 4.88E+0
deprived]
GWP = Global warming potential; ODP = Depletion potential of the stratospheric ozone layer; AP = Acidification potential of land and water; EP =
Caption Eutrophication potential; POCP = Formation potential of tropospheric ozone photochemical oxidants; ADPE = Abiotic depletion potential for non-
fossil resources; ADPF = Abiotic depletion potential for fossil resources; WDP = Water (user) deprivation potential
RESULTS OF THE LCA - INDICATORS TO DESCRIBE RESOURCE USE according to EN 15804+A2:
declared unit and product
Indicator Unit A1 A2 A3 A4 C1 C2 C3 C4 D
PERE [MJ] 1.10E+3 3.91E+1 3.91E+4 1.66E+1 8.28E+0 6.17E+0 1.16E+1 3.80E+0 -5.29E+1
PERM [MJ] 0.00E+0 0.00E+0 0.00E+0 0.00E+0 0.00E+0 0.00E+0 0.00E+0 0.00E+0 0.00E+0
PERT [MJ] 0.00E+0 0.00E+0 3.90E+4 0.00E+0 0.00E+0 0.00E+0 0.00E+0 0.00E+0 0.00E+0
PENRE [MJ] 0.00E+0 0.00E+0 0.00E+0 0.00E+0 0.00E+0 0.00E+0 0.00E+0 0.00E+0 0.00E+0
PENRM [MJ] 1.10E+3 3.91E+1 7.81E+4 1.66E+1 8.28E+0 6.17E+0 1.16E+1 3.80E+0 -5.29E+1
PENRT [MJ] 0.00E+0 0.00E+0 0.00E+0 0.00E+0 0.00E+0 0.00E+0 0.00E+0 0.00E+0 0.00E+0
SM [kg] 1.90E+4 2.94E+3 2.19E+4 1.51E+3 6.95E+1 5.06E+2 2.02E+2 2.10E+2 -4.69E+3
RSF [MJ] 0.00E+0 0.00E+0 0.00E+0 0.00E+0 0.00E+0 0.00E+0 0.00E+0 0.00E+0 0.00E+0
NRSF [MJ] 0.00E+0 6.99E+1 1.35E+3 0.00E+0 0.00E+0 0.00E+0 0.00E+0 0.00E+0 0.00E+0
FW [m³] 7.53E+0 2.00E-1 1.28E+1 9.37E-2 2.02E-2 3.39E-2 2.33E-2 2.72E-1 -8.89E-1
PERE = Use of renewable primary energy excluding renewable primary energy resources used as raw materials; PERM = Use of
renewable primary energy resources used as raw materials; PERT = Total use of renewable primary energy resources; PENRE = Use of
non-renewable primary energy excluding non-renewable primary energy resources used as raw materials; PENRM = Use of non-
Caption
renewable primary energy resources used as raw materials; PENRT = Total use of non-renewable primary energy resources; SM = Use
of secondary material; RSF = Use of renewable secondary fuels; NRSF = Use of non-renewable secondary fuels; FW = Use of net fresh
water
RESULTS OF THE LCA – WASTE CATEGORIES AND OUTPUT FLOWS according to EN 15804+A2:
declared unit and product
Indicator Unit A1 A2 A3 A4 C1 C2 C3 C4 D
HWD [kg] 1.46E+0 4.16E-3 6.57E+1 4.10E-2 2.55E-3 0.00E+0 7.06E-2 5.17E-2 -4.82E-1
NHWD [kg] 3.12E+3 1.03E-1 2.11E+3 2.84E-1 8.69E+0 0.00E+0 1.73E+1 4.18E+3 -8.73E+2
RWD [kg] 4.97E-5 1.02E-6 1.60E-5 2.29E-6 2.25E-7 0.00E+0 2.63E-6 1.34E-6 -1.03E-5
CRU [kg] 0.00E+0 0.00E+0 0.00E+0 0.00E+0 0.00E+0 0.00E+0 0.00E+0 0.00E+0 0.00E+0
MFR [kg] 0.00E+0 0.00E+0 1.09E+2 0.00E+0 0.00E+0 0.00E+0 8.50E+2 0.00E+0 0.00E+0
MER [kg] 0.00E+0 0.00E+0 0.00E+0 0.00E+0 0.00E+0 0.00E+0 0.00E+0 0.00E+0 0.00E+0
EEE [MJ] 0.00E+0 0.00E+0 0.00E+0 0.00E+0 0.00E+0 0.00E+0 0.00E+0 0.00E+0 0.00E+0
EET [MJ] 0.00E+0 0.00E+0 0.00E+0 0.00E+0 0.00E+0 0.00E+0 0.00E+0 0.00E+0 0.00E+0
HWD = Hazardous waste disposed; NHWD = Non-hazardous waste disposed; RWD = Radioactive waste disposed; CRU = Components
Caption for re-use; MFR = Materials for recycling; MER = Materials for energy recovery; EEE = Exported electrical energy; EET = Exported
thermal energy
RESULTS OF THE LCA – additional impact categories according to EN 15804+A2-optional:
[declared unit and product]
Indicator Unit A1 A2 A3 A4 C1 C2 C3 C4 D
[Disease
PM 1.06E-4 1.37E-5 1.32E-4 7.88E-6 6.41E-7 2.84E-6 2.36E-6 3.48E-6 -2.82E-5
Incidence]
[kBq U235-
IRP 5.21E+1 1.32E+1 3.70E+1 6.60E+0 3.34E-1 2.22E+0 1.20E+0 4.98E-1 -4.49E+0
Eq.]
ETP-fw [CTUe] 8.25E+4 2.27E+3 4.57E+4 1.08E+3 9.06E+1 3.88E+2 7.31E+1 3.22E+2 -9.35E+3
HTP-c [CTUh] 1.25E-5 7.85E-8 7.61E-6 3.38E-8 4.79E-8 1.19E-8 1.38E-9 3.60E-8 -2.41E-6
HTP-nc [CTUh] 6.04E-5 2.29E-6 2.65E-5 1.14E-6 6.99E-8 4.10E-7 8.44E-8 2.84E-6 -9.28E-6
SQP [-] 5.48E+3 2.30E+3 4.25E+5 1.55E+3 1.03E+1 5.80E+2 8.30E+0 2.45E+2 -1.25E+3
PM = Potential incidence of disease due to PM emissions; IR = Potential Human exposure efficiency relative to U235; ETP-fw = Potential
Caption comparative Toxic Unit for ecosystems; HTP-c = Potential comparative Toxic Unit for humans (cancerogenic); HTP-nc = Potential
comparative Toxic Unit for humans (not cancerogenic); SQP = Potential soil quality index
Disclaimer 1 – for the indicator “Potential Human exposure efficiency relative to U235”.This impact category deals
mainly with the eventual impact of low dose ionizingradiation on human health of the nuclear fuel cycle. It does
not consider effects due to possiblenuclear accidents, occupational exposure or radioactive waste disposal in
undergroundfacilities. Potential ionizing radiation from the soil, from radon and from some construction materials
is also not measured by this indicator.
Disclaimer 2 – for the indicators “abiotic depletion potential for non-fossil resources”, “abiotic depletion potential
for fossil resources”, “water (user) deprivation potential, deprivation-weighted water consumption”, “potential
comparative toxic unit for ecosystems”, “potential comparative toxic unit for humans – cancerogenic”, “Potential
comparative toxic unit for humans - not cancerogenic”, “potential soil quality index”. The results of this
environmental impact indicator shall be used with care as theuncertainties on these results are high as there is
limited experience with the indicator.
References
AIB
Association of Issuing Bodies. European Residual SCI
Mixes. Results of the calculation of Residual Mixes for SteelConstruction.info, The recycling and reuse
the calendar year 2020. https://www.aib- survey.
net.org/facts/european-residual-mix https://www.steelconstruction.info/The_recycling_and_
reuse_survey. Access: August 2022.
AISI
American Iron and Steel Institute. Steel sustainability in SimaPro
the construction market. https://www.steel.org/wp- SimaPro software, v. 9.2.0.1.
content/uploads/2020/09/Steel-Sustainability-in-
Construction-Fact-Sheet.pdf WSA
World steel association. Life cycle inventory (LCI)
Ecoinvent study 2020 data release. Seventh global LCI study for
Ecoinvent database v. 3.7.1 steel products. May 2021; p.19.
EEA Standards, Regulation
EEA Report No 13/2019Technical guidance to prepare AWS D1.1
national emission inventories. AWS D1.1: Structural Welding Code—Steel. 2000.
https://www.eea.europa.eu/publications/emep-eea-
guidebook-2019 BSK 07
The Housing Authority's handbook on steel structures,
EPLCA BSK 07 (Boverkets handbok om stålkonstruktioner,
European Platform on Life Cycle Assessment, BSK 07), Boverket 2007.
Environmental Footprint,
https://eplca.jrc.ec.europa.eu/EnvironmentalFootprint.h DIN 15018
tml DIN 15018-3. Cranes; principles relating to steel
structures; design of cranes on vehicles. 1984.
IBU Instruction
GENERAL INSTRUCTIONS for the EPD programme DIN 18800-7
of Institut Bauen und Umwelt e.V., v. 2.0, 2021. DIN 18800-7. Steel structures - Part 7: Execution and
constructor's qualification. 2008.
PCR Part A
IBU. Product Category Rules for Building-Related DIN 19704
Products and Services. Part A: Calculation Rules for DIN 19704. Hydraulic steel structures - Part 1: Criteria
the Life Cycle As-sessment and Requirements on the for design and calculation; Hydraulic steel structures -
Project Re-port according to EN 15804+A2:2019; v Part 2: Design and manufacturing. 2014.
1.2, 2021.
DIN 24537
PCR Part B DIN 24537. Grating type. 2007.
IBU. PCR Guidance-Texts for Building-Related
Products and Services. Part B: Requirements on the
EPD for Structural steels, v. 1.6, 2017.
6 Environmental Product Declaration Mostostal – Steel structures, pallets and platform gratings + coating (optional)
EN 10346 EN ISO 14025
EN 10346:2015. Continuously hot-dip coated steel flat EN ISO 14025:2010, Environmental labels and
products for cold forming – Technical delivery declarations. Type III environmental declarations.
conditions. Principles and procedures.
EN 1090-1 EU No 305/2011
EN 1090-1:2009+A1:2011 Execution of steel Regulation (EU) No 305/2011 - construction products -
structures and aluminium structures - Part 1: of 9 March 2011 laying down harmonised conditions
Requirements for conformity assessment of structural for the marketing of construction products and
components. repealing Council Directive 89/106/EEC (Latest
update: 2017).
EN 1090-2
EN 1090-2:2018 Execution of steel structures and EN ISO 1461 (DIN 50976)
aluminium structures - Part 2: Technical requirements PN-EN ISO 1461:2011 Hot dip galvanized coatings on
for steel structure. fabricated iron and steel articles. Specifications and
test methods (Polish version). DIN 50976. Protection
EN 15804 against Corrosion - Coatings on iron and steel
EN 15804:2012+A2:2019/AC:2021. Sustainability of components applied by hot dip zinc coating -
construction works - Environmental product Requirements and testing, 1989.
declarations - Core rules for the product category of
construction products.
7 Environmental Product Declaration Mostostal – Steel structures, pallets and platform gratings + coating (optional)
Publisher
Institut Bauen und Umwelt e.V. Tel +49 (0)30 3087748- 0
Hegelplatz 1 Fax +49 (0)30 3087748- 29
10117 Berlin Mail info@ibu-epd.com
Germany Web www.ibu-epd.com
Programme holder
Institut Bauen und Umwelt e.V. Tel +49 (0)30 - 3087748- 0
Hegelplatz 1 Fax +49 (0)30 – 3087748 - 29
10117 Berlin Mail info@ibu-epd.com
Germany Web www.ibu-epd.com
Author of the Life Cycle
Assessment Tel +48 586610708
SGS Polska sp. z o.o. Fax +48 586610707
Jana Kazimierza 3 Mail ilona.olsztynska@sgs.com
01-248 Warszawa Web https://www.sgs.pl/
Poland
Owner of the Declaration
Mostostal Siedlce Limited liability Tel +48256439467
company LP Fax +48256439657
Terespolska 12 Mail mostostal-siedlce@polimex.pl
08-110 Siedlce Web www.mostostal.siedlce.pl
Poland
