ENVIRONMENTAL PRODUCT DECLARATION
as per ISO 14025 and EN 15804+A2
Owner of the Declaration Hansgrohe Group
Publisher Institut Bauen und Umwelt e.V. (IBU)
Programme holder Institut Bauen und Umwelt e.V. (IBU)
Declaration number EPD-HAN-20240193-ICC1-EN
Issue date 26.09.2024
Valid to 25.09.2029
Toilets
Hansgrohe Group
www.ibu-epd.com | https://epd-online.com
1. General Information
Hansgrohe Group Toilets
Programme holder Owner of the declaration
IBU – Institut Bauen und Umwelt e.V. Hansgrohe Group
Hegelplatz 1 Auestr. 5-9
10117 Berlin 77761 Schiltach
Germany Germany
Declaration number Declared product / declared unit
EPD-HAN-20240193-ICC1-EN One piece of an average ceramic toilet incl. packaging
This declaration is based on the product category rules: Scope:
Sanitary ceramics, 01.08.2021 This average EPD is valid for the product group of ceramic toilets of the
(PCR checked and approved by the SVR) hansgrohe brand sold on the European market. The products are
produced in Italy and Egypt.
The owner of the declaration shall be liable for the underlying information
Issue date and evidence; the IBU shall not be liable with respect to manufacturer
information, life cycle assessment data and evidences.
26.09.2024
The EPD was created according to the specifications of EN 15804+A2. In
the following, the standard will be simplified as EN 15804.
Valid to
25.09.2029 Verification
The standard EN 15804 serves as the core PCR
Independent verification of the declaration and data according to ISO
14025:2011
internally X externally
Dipl.-Ing. Hans Peters
(Chairman of Institut Bauen und Umwelt e.V.)
Florian Pronold Dr Naeem Adibi,
(Managing Director Institut Bauen und Umwelt e.V.) (Independent verifier)
1 Environmental Product Declaration - Hansgrohe Group - Toilets
2. Product
Name Value Unit
2.1 Product description/Product definition
Ceramic 91 - 94 %
The product group of toilets refers to ceramic articles in various
Steel < 1 %
sizes and designs (excluding E-toilets or bundles).
Plastic < 1 %
The basic material of ceramics consists of natural raw materials Other <1 %
such as clay, kaolin, quartz and feldspar that are mixed Cardboard and paper (packaging) 6 - 8 %
according to a specific recipe. A glaze protects the products
Polyethylene (packaging) < 1 %
from external influences.
This product contains substances listed in the candidate list
Depending on the model, additional components (e. g. made of (date: 12.12.2023) exceeding 0.1 percentage by mass: no.
plastic or metals) may be included in the scope of delivery.
For the placing on the market of the product in the European This product/article/at least one partial article contains other
Union/European Free Trade Association (EU/EFTA) (with the CMR substances in categories 1A or 1B which are not on the
exception of Switzerland) Regulation (EU) No. 305/2011 (CPR) candidate list, exceeding 0.1 percentage by mass: no.
applies. The product needs a declaration of performance taking
into consideration Biocide products were added to this construction product or it
has been treated with biocide products (this then concerns a
• EN 997:2012, WC pans and WC suites with integral trap
treated product as defined by the (EU) Ordinance on Biocide
and the CE-marking.
Products No. 528/2012): yes.
In order to get the desired viscosity, fungicides are added to the
For the application and use the respective national provisions
glaze. These burn completely during the firing process and are
apply.
not part of the final product.
2.6 Manufacture
2.2 Application
As typical sanitary installations toilets are part of the bathroom
and support the water-based physical hygiene. They are
connected to a cistern to provide the hygiene function.
2.3 Technical Data
Constructional data
Name Value Unit
Width 360 mm
Length 540 mm
Height 320 mm
Maximum heat resistance temperature (if
1100 °C
relevant)
Vol.-
Maximum water absorption (if relevant) 6
%
Resistance to chemicals and staining passed -
Resistance to temperature change passed -
Performance data of the product in accordance with the
declaration of performance with respect to its essential
characteristics according to
• EN 997:2012, WC pans and WC suites with integral No. 1: The "slip" is prepared by mixing raw materials and water.
trap. No. 2: The moulds are made by gypsum.
No. 3: The "slip" is filled into the moulds.
2.4 Delivery status No. 4: The pieces are drying.
The toilets are delivered singularly packaged. The packaging is No. 5: Glaze is prepared.
customized to the size of the product and supplies. The No. 6: Glaze is applied.
products with the smallest and the largest volume have No. 7: The pieces are fired in the kiln.
dimensions between 390x570x360 mm and 391x580x391 mm. No. 8: The pieces are inspected for any defects.
No. 8a: Some parts are reworked, e. g. by grinding certain
2.5 Base materials/Ancillary materials areas.
The material composition (incl. packaging and additional parts) No. 8b: Some parts are refired.
of toilets are as follows: No. 9: The products are packed.
2.7 Environment and health during manufacturing
Hansgrohe SE tries to keep the impact on people and the
environment as low as possible when manufacturing its
products.
For example, state-of-the-art systems (e. g. kilns) are used in
the production process of sanitary ceramics and application of
2 Environmental Product Declaration - Hansgrohe Group - Toilets
the glaze is partially carried out by robots. (non-combustible without combustible building materials) in
In addition, all production sites are certified according to the accordance with EN-13501-1.
ISO 9001 (quality), KIWA and NF.
Fire protection
2.8 Product processing/Installation Name Value
Mounting of wall hung toilets is carried out in combination with a Building material class A1
cistern system, which usually includes attachment parts. Burning droplets -
Additional required parts are included in the scope of delivery.
Smoke gas development -
• Shorten the drain pipes (tools: pencil, meter stick, saw,
file).
Water
• Add the sound insulation mat.
If a room in which the products offered by Hansgrohe are
• Insert the drain pipes (tools: grease).
installed is flooded with water, the products are not affected in
• The toilet is fixed to the mounting parts of the cistern
their function.
system (tools: hexagonal offset screwdriver).
There will be no environmental impact.
• Sealing is done with silicone (tools: silicone syringe).
2.9 Packaging Mechanical destruction
Minor mechanical damages have no effect on product function.
For product protection the toilets are individually packed in a
If the glazed surface of the ceramic is severely destroyed by a
printed cardboard box. The inlay of the packaging consists of
mechanical stress and the glaze flakes off, there is a very small
folded cardboard or plastic bags, depending on the product.
possibility of water uptake as usual with ceramic products. In
The packaging can be fully recycled. All packaged products fit
this event the products may need to be replaced.
on a reusable euro pallet.
2.14 Re-use phase
2.10 Condition of use
The toilets are not taken back by the manufacturer for the
To protect the toilets and make them durable, the ceramic
purpose of reuse. Users can disassemble the products
material is glazed. If used as intended, there are no unhealthy
repeatedly within the reference utilization period and reuse
contaminants caused by the sanitary ceramics. To ensure the
them elsewhere.
longevity of the product, it should be cleaned regularly.
2.15 Disposal
2.11 Environment and health during use
The waste code of the product is AVV 17 01 03.
Our products do not emission any contaminants or substances
Disassembly of the products consists of the same steps as
that are harmful to the environment or health during the use
assembly, in reverse order. Due to the disassembly process,
phase.
the individual parts may be collected separately.
2.12 Reference service life The ceramic material will mostly be disposed via inert landfills.
The quality and durability of our toilets is designed for a product All metal components can be recycled (as scrap). All plastic
life of about 20 years. Which on average is approximately the components have a high calorific value and can be sent for
duration of use by the consumers. thermal recycling.
In countries where no thermal recycling or substance recycling
All products in the scope of this study have a 20-year warranty. is established, disposal takes place via the waste incineration
plant.
2.13 Extraordinary effects 2.16 Further information
Fire Additional information about our products can be found at
Sanitary ceramics are classified as building material class A1 https://www.hansgrohe.com.
3. LCA: Calculation rules
3.1 Declared Unit
The results of this EPD are valid for the following declared unit: 3.2 System boundary
one (1) wall hung toilet including packaging, used in This average EPD follows the EPD type "cradle to grave". The
accordance with the manufacturer's recommendations for a 20- following life cycle modules are declared:
year life, following the manufacturer's operating instructions.
The wall frame and toilet lid are excluded. Modules A1-A3
The product stage begins with considering the production of the
Weighted averaging based on forecast sales volumes is chosen necessary raw materials and energies, including all
as the basis for creating the environmental profile. 9 different corresponding upstream chains and the actual procurement
toilets were considered. transports. Furthermore, the entire manufacturing phase was
mapped, including the treatment of production waste until the
Declared unit
end-of-waste status (EoW) was reached. Location-specific
Name Value Unit
electricity mixes were considered.
Declared unit 1 piece
Declared unit (ceramic mass) 0.0247 t Module A4
Mass (product) 24.858 kg Distribution transports (A4) to the customers were considered.
Mass (packaging) 1.774 kg
Module A5
This module covers the installation process with the
corresponding packaging waste generated that needs to be
disposed of.
3 Environmental Product Declaration - Hansgrohe Group - Toilets
datasets were not available.
Module B2
Maintenance expenses are declared in this module and consist 3.6 Data quality
of weekly cleaning expenses for these products. The data for the examined products was captured on the basis
of evaluations of internal production and environmental data,
Module B1, B3-B7 the collection of LCA relevant data within the supply chain, as
These modules were considered, but evaluated as not relevant well as the evaluation of relevant data for the energy supply.
and therefore considered as zero. The collected data were checked for plausibility and
consistency. Good representativity can be assumed.
Modules C1-C4
3.7 Period under review
The modules include the environmental impacts for dismantling
and the treatment of the waste fractions until the end-of-waste Life cycle assessment data were collected for a 12-month
status (EoW) is reached, including the associated transports at period in the years 2022 and 2023.
the end of the product life cycle.
3.8 Geographic Representativeness
Land or region, in which the declared product system is
Module D
manufactured, used or handled at the end of the product´s
Identification of the benefits and costs of the product outside
lifespan: Global
the system boundary. For plastics, these consist of energy
credits from thermal utilization in the form of the average
European electricity mix or thermal energy from natural gas. 3.9 Allocation
Recycling of steel results in material credits.
For the production of the ceramic, supplier-data was gathered
for a 12-month period and then allocated to the products under
3.3 Estimates and assumptions
consideration by weight. This applies to the material inputs and
For the incineration with energy recovery (thermal and electric)
outputs as well as energy demands.
of waste, an r1 value of >0.6 is assumed. The net efficiency for
The composition of the products under consideration was
the average waste incinerated is 44 %.
modelled based on BOMs. Therefore, no further allocation was
necessary.
All products are assumed to be first shipped to the warehouse
Allocation of co-production processes is not relevant.
and then shipped to the customers. This is a conservative
assumption since some products are shipped directly from the
Recycled materials enter the product system without any loads
manufacturing site to the customer. However, no reliable data is
in the modules A1-A3 and therefore do not generate any
available.
benefits in module D.
3.4 Cut-off criteria
Loads and benefits beyond the system boundary resulting from
The effect associated with the neglected mass shares is less
production waste in module A1-A3 are cut-off.
than 5 % of the effect categories per module. The minimum
limit of 1 % total mass and the use of renewable and non-
Loads and benefits beyond the system boundary resulting from
renewable primary energy is not exceeded.
the treatment of packaging materials in module A5 and the
3.5 Background data product in the C-modules are assigned to module D.
The LCA software LCA for Experts 10.7 was used to model the
life cycle. The entire manufacturing process, as well as energy
consumption, were modelled on the basis of manufacturer-
3.10 Comparability
specific data.
Basically, a comparison or an evaluation of EPD data is only
possible if all the data sets to be compared were created
However, generic background datasets were used for the
according to EN 15804 and the building context, respectively
upstream and downstream processes. The majority of the
the product-specific characteristics of performance, are taken
background datasets used were taken from the content version
into account. The background database used is LCA for
2023.2 of the Sphera Managed LCA Content database.
Experts content version 2023.2.
Ecoinvent Version 3.9.1 datasets were only used when suitable
4. LCA: Scenarios and additional technical information
Transport to the building site (A4)
Characteristic product properties of biogenic carbon
Name Value Unit
Transport distance (truck) 1915 km
Information on describing the biogenic carbon content at
factory gate Capacity utilisation (including empty runs) (truck) 55 %
Note: 1 kg of biogenic carbon is equivalent to 44/12 kg of CO . Transport distance (ship) 914 km
2
Name ValueUnit Installation into the building (A5)
Biogenic carbon content in product kg Name ValueUnit
C
Silicone 0.052 kg
Biogenic carbon content in accompanying kg
0.718 Output substances following waste treatment on
packaging C 1.744 kg
site (packaging materials)
4 Environmental Product Declaration - Hansgrohe Group - Toilets
Maintenance (B2) Reference service life
Name Value Unit Name Value Unit
Information on maintenance (weekly Life Span according to the manufacturer 20 a
-
cleaning with soapy water)
End of life (C1-C4)
Maintenance cycle 1043 Number/RSL
Water consumption 0.522 m3 Name Value Unit
Collected as mixed construction waste 24.858 kg
Other resources (soap) 7.827 kg
Recycling 0.037 kg
Information on maintenance (replacement
of silicone) Landfilling 24.821 kg
Maintenance cycle 1 Number/RSL
Reuse, recovery and/or recycling potentials (D), relevant
Other resources (silicone) 0.052 kg scenario information
Name Value Unit
5 Environmental Product Declaration - Hansgrohe Group - Toilets
5. LCA: Results
The LCA results of the module B2 are declared for the service life of 20 years.
DESCRIPTION OF THE SYSTEM BOUNDARY (X = INCLUDED IN LCA; MND = MODULE OR INDICATOR NOT DECLARED; MNR
= MODULE NOT RELEVANT)
Benefits and
Construction loads beyond
Product stage Use stage End of life stage
process stage the system
boundaries
la ire ta m w a Ry lp p u s tro p s n a rT g n iru tc a fu n a M e h t m o rf tro p s n a rTe tis e h t o t e ta g y lb m e s s A e s U e c n a n e tn ia M ria p e R tn e m e c a lp e R tn e m h s ib ru fe R y g re n e la n o ita re p Oe s u re ta w la n o ita re p Oe s u n o itc u rts n o c -e Dn o itilo m e d tro p s n a rT g n is s e c o rp e ts a W la s o p s iD -e s u e R-y re v o c e R-g n ilc y c e Rla itn e to p
A1 A2 A3 A4 A5 B1 B2 B3 B4 B5 B6 B7 C1 C2 C3 C4 D
X X X X X X X X X X X X X X X X X
RESULTS OF THE LCA - ENVIRONMENTAL IMPACT according to EN 15804+A2: 1 piece toilet
Parameter Unit A1-A3 A4 A5 B1 B2 B3 B4 B5 B6 B7 C1 C2 C3 C4 D
GWP-total kg CO 2 eq 4E+01 5.44E+003.04E+00 0 2.48E+01 0 0 0 0 0 0 2.47E-01 3.68E-01 3.74E-01 -2.88E-02
GWP-fossil kg CO 2 eq 4.25E+015.39E+00 4.1E-01 0 1.87E+01 0 0 0 0 0 0 2.45E-01 3.67E-01 3.72E-01 -2.88E-02
GWP- -2.63E
biogenic kg CO 2 eq +00 0 2.63E+00 0 0 0 0 0 0 0 0 0 0 0 0
GWP-luluc kg CO 2 eq 4.49E-02 4.79E-02 7.25E-04 0 6.04E+00 0 0 0 0 0 0 2.26E-03 1.2E-03 1.16E-03 -1.88E-06
kg CFC11
ODP 4.23E-07 6.89E-13 2.05E-12 0 1.09E-06 0 0 0 0 0 0 3.17E-14 4.46E-12 9.56E-13 -2.26E-13
eq
AP mol H+ eq 1.86E-01 4.22E-02 1.37E-03 0 6.77E-02 0 0 0 0 0 0 1.05E-03 1.2E-03 2.65E-03 -3.6E-05
EP-
kg P eq 1.06E-03 1.9E-05 8.59E-07 0 5.9E-04 0 0 0 0 0 0 8.91E-07 1.36E-06 1.98E-06 -4.67E-08
freshwater
EP-marine kg N eq 5.48E-02 2.05E-02 3.48E-04 0 1.54E-02 0 0 0 0 0 0 4.91E-04 4.56E-04 6.85E-04 -1.05E-05
EP-terrestrial mol N eq 5.88E-01 2.27E-01 3.79E-03 0 1.84E-01 0 0 0 0 0 0 5.49E-03 4.98E-03 7.54E-03 -1.13E-04
kg
POCP NMVOC 1.45E-01 4.1E-02 1.08E-03 0 6.14E-02 0 0 0 0 0 0 9.49E-04 1.02E-03 2.07E-03 -2.94E-05
eq
ADPE kg Sb eq 4.55E-05 3.45E-07 7E-06 0 2.81E-05 0 0 0 0 0 0 1.62E-08 4.56E-08 1.73E-08 -2.07E-09
ADPF MJ 6.67E+027.34E+016.88E+00 0 4.6E+02 0 0 0 0 0 0 3.32E+006.79E+005.04E+00 -5.32E-01
m3 world
WDP eq 3.72E+00 6.29E-02 1.26E-01 0 6.75E+00 0 0 0 0 0 0 2.95E-03 5.51E-02 4.07E-02 -2.74E-03
deprived
GWP = Global warming potential; ODP = Depletion potential of the stratospheric ozone layer; AP = Acidification potential of land and water; EP =
Eutrophication potential; POCP = Formation potential of tropospheric ozone photochemical oxidants; ADPE = Abiotic depletion potential for non-fossil
resources; ADPF = Abiotic depletion potential for fossil resources; WDP = Water (user) deprivation potential)
RESULTS OF THE LCA - INDICATORS TO DESCRIBE RESOURCE USE according to EN 15804+A2: 1 piece toilet
Parameter Unit A1-A3 A4 A5 B1 B2 B3 B4 B5 B6 B7 C1 C2 C3 C4 D
PERE MJ 4.87E+015.14E+00 3.2E+01 0 9.71E+01 0 0 0 0 0 0 2.42E-01 3.15E+00 8.15E-01 -1.54E-01
-2.88E
PERM MJ 2.88E+01 0 0 0 0 0 0 0 0 0 0 0 0 0
+01
PERT MJ 7.75E+015.14E+003.23E+00 0 9.71E+01 0 0 0 0 0 0 2.42E-01 3.15E+00 8.15E-01 -1.54E-01
PENRE MJ 6.66E+027.37E+015.85E+00 0 4.6E+02 0 0 0 0 0 0 3.33E+006.79E+005.05E+00 -5.32E-01
PENRM MJ 2.32E+00 0 1.03E+00 0 0 0 0 0 0 0 0 0 0 0 0
PENRT MJ 6.68E+027.37E+016.88E+00 0 4.6E+02 0 0 0 0 0 0 3.33E+006.79E+005.05E+00 -5.32E-01
SM kg 1.52E+00 0 0 0 0 0 0 0 0 0 0 0 0 0 1.92E-01
RSF MJ 0 0 0 0 0 0 0 0 0 0 0 0 0 0 0
NRSF MJ 0 0 0 0 0 0 0 0 0 0 0 0 0 0 0
FW m3 1.09E-01 5.63E-03 4.37E-03 0 1.59E-01 0 0 0 0 0 0 2.65E-04 2.58E-03 1.25E-03 -1.25E-04
PERE = Use of renewable primary energy excluding renewable primary energy resources used as raw materials; PERM = Use of renewable primary
energy resources used as raw materials; PERT = Total use of renewable primary energy resources; PENRE = Use of non-renewable primary energy
excluding non-renewable primary energy resources used as raw materials; PENRM = Use of non-renewable primary energy resources used as raw
materials; PENRT = Total use of non-renewable primary energy resources; SM = Use of secondary material; RSF = Use of renewable secondary fuels;
NRSF = Use of non-renewable secondary fuels; FW = Use of net fresh water
RESULTS OF THE LCA – WASTE CATEGORIES AND OUTPUT FLOWS according to EN 15804+A2:
1 piece toilet
Parameter Unit A1-A3 A4 A5 B1 B2 B3 B4 B5 B6 B7 C1 C2 C3 C4 D
HWD kg 2.81E-05 2.28E-10 2.15E-10 0 8.53E-03 0 0 0 0 0 0 1.03E-11 -3.91E-10 1.16E-10 -2.85E-11
NHWD kg 7.26E+00 1.1E-02 8.35E-02 0 8.13E-01 0 0 0 0 0 0 5.08E-04 3.97E-03 2.48E+01 -2.63E-04
RWD kg 1.89E-03 1.36E-04 3.53E-04 0 4.48E-03 0 0 0 0 0 0 6.24E-06 8.08E-04 5.76E-05 -4.1E-05
CRU kg 0 0 0 0 0 0 0 0 0 0 0 0 0 0 0
6 Environmental Product Declaration - Hansgrohe Group - Toilets
MFR kg 0 0 1.74E+00 0 0 0 0 0 0 0 0 0 3.73E-02 0 0
MER kg 0 0 0 0 0 0 0 0 0 0 0 0 0 0 0
EEE MJ 0 0 1.02E-03 0 1.35E-01 0 0 0 0 0 0 0 0 0 0
EET MJ 0 0 1.81E-03 0 2.46E-01 0 0 0 0 0 0 0 0 0 0
HWD = Hazardous waste disposed; NHWD = Non-hazardous waste disposed; RWD = Radioactive waste disposed; CRU = Components for re-use;
MFR = Materials for recycling; MER = Materials for energy recovery; EEE = Exported electrical energy; EET = Exported thermal energy
RESULTS OF THE LCA – additional impact categories according to EN 15804+A2-optional:
1 piece toilet
Parameter Unit A1-A3 A4 A5 B1 B2 B3 B4 B5 B6 B7 C1 C2 C3 C4 D
Disease
PM 2.47E-06 2.61E-07 1.33E-08 0 3.33E-06 0 0 0 0 0 0 5.95E-09 6.55E-09 3.26E-08 -3.06E-10
incidence
kBq U235
IR 4.5E-01 2.02E-02 5.76E-02 0 2.2E+00 0 0 0 0 0 0 9.3E-04 1.34E-01 6.69E-03 -6.82E-03
eq
ETP-fw CTUe 1.24E+025.25E+01 2.1E+00 0 1.72E+02 0 0 0 0 0 0 2.38E+002.64E+002.76E+00 -7.4E-02
HTP-c CTUh 8.46E-09 1.06E-09 1.92E-09 0 2.39E-08 0 0 0 0 0 0 4.83E-11 9.95E-11 4.2E-10 -5.89E-12
HTP-nc CTUh 2.76E-07 4.68E-08 2.19E-07 0 5.48E-07 0 0 0 0 0 0 2.15E-09 2.3E-09 4.42E-08 -1.45E-10
SQP SQP 1.72E+022.94E+011.25E+01 0 3.3E+02 0 0 0 0 0 0 1.39E+002.71E+001.21E+00-1.02E-01
PM = Potential incidence of disease due to PM emissions; IR = Potential Human exposure efficiency relative to U235; ETP-fw = Potential comparative
Toxic Unit for ecosystems; HTP-c = Potential comparative Toxic Unit for humans (cancerogenic); HTP-nc = Potential comparative Toxic Unit for humans
(not cancerogenic); SQP = Potential soil quality index
Disclaimer 1 – for the indicator “Potential Human exposure efficiency relative to U235”. This impact category deals mainly with the
eventual impact of low-dose ionizing radiation on human health of the nuclear fuel cycle. It does not consider effects due to possible
nuclear accidents, occupational exposure or radioactive waste disposal in underground facilities. Potential ionizing radiation from the
soil, radon and from some construction materials is also not measured by this indicator.
Disclaimer 2 – for the indicators “abiotic depletion potential for non-fossil resources”, “abiotic depletion potential for fossil resources”,
“water (user) deprivation potential, deprivation-weighted water consumption”, “potential comparative toxic unit for ecosystems”,
“potential comparative toxic unit for humans – cancerogenic”, “Potential comparative toxic unit for humans - not cancerogenic”,
“potential soil quality index”. The results of this environmental impact indicator shall be used with care as the uncertainties on these
results are high as there is limited experience with the indicator.
6. LCA: Interpretation
maintenance (module B2), as well as the energy inputs (gas
The figure above shows the dominance analysis over the and electricity) for the production of the ceramic.
considered modules. It can be seen here that the production
phase (modules A1-A3) as well as the maintenance (module Variability
B2) dominate the LCA results over the life cycle. GWP-biogenic Module B2 is the same for all products. The results in the other
is negative in modules A1-A3 due to biogenic carbon stored in modules are mainly dependend on the weight of the products
the packaging (cardboard and paper). The biogenic carbon and the production location.
balance is offset with the treatment of the packaging in module
A5. The weight of the products (incl. packaging) varies between 24
The datasets that have relatively high contributions to many and 28.1 kg (ceramic mass between 22.2 and 26.3 kg). In
included indicators are the dataset used for the soap in for general, heavier products have higher potential environmental
7 Environmental Product Declaration - Hansgrohe Group - Toilets
impacts during production (A1-A3) and end-of-life (C-modules) Keeping product weight constant there still is variability which is
since more materials and energies are required. due to different production conditions of the two sites and
associated energy mixes.
7. Requisite evidence
8 Environmental Product Declaration - Hansgrohe Group - Toilets
8. References
(Federal Law Gazette 2833)
Standards
CPR
EN 13501-1 Construction Products Regulation
EN 13501-1:2019-05, Fire classification of construction
products and building elements - Part 1: Classification using Candidate list
data from reaction to fire tests Candidate List of substances of very high concern for
Authorisation, published in accordance with Article 59(10) of the
EN 14688 REACH Regulation. Helsinki: European Chemicals Agency
EN 14688:2018-12, Sanitary appliances - Wash basins -
Functional requirements and test methods IBU 2021
Institut Bauen und Umwelt e.V.: General Instructions for the
EN 15804 EPD programme of Institut Bauen und Umwelt e.V., Version
EN 15804:2012+A2:2019 + AC:2021, Sustainability of 2.0, Berlin: Institut Bauen und Umwelt e.V., 2021 www.ibu-
construction works — Environmental Product Declarations — epd.com
Core rules for the product category of construction products.
Managed LCA Content
ISO 9001 Managed LCA Content. Content Version 2023.2. Leinfeld-
ISO 9001:2015-11, Quality management systems - Echterdingen: Sphera Solutions GmbH.
Requirements
PCR part A
Product Category Rules for Building-Related Products and
ISO 14025 Services. Part A: Calculation Rules for the Life Cycle
ISO 14025:2006-07, Environmental labels and declarations - Assessment and Requirements on the Project Report, Version
Type III environmental declarations - Principles and procedures 1.3. Berlin: Institut Bauen und Umwelt e.V. (ed.), 2021.
Further references PCR: Sanitary ceramics
PCR Guidance-Texts for Building-Related Products and
AVV Services. Part B: Requirements on the EPDs for Sanitary
Waste Catalogue Ordinance (Abfallverzeichnis-Verordnung - Ceramics, Version 4. Berlin: Institut Bauen und Umwelt e.V.
AVV) of 10 December 2001 (Federal Law Gazette I p. 3379), (publisher.), 19.10.2023.
last amended by Article 2 of the Ordinance of 24 July 2002
9 Environmental Product Declaration - Hansgrohe Group - Toilets
Publisher
Institut Bauen und Umwelt e.V. +49 (0)30 3087748- 0
Hegelplatz 1 info@ibu-epd.com
10117 Berlin www.ibu-epd.com
Germany
Programme holder
Institut Bauen und Umwelt e.V. +49 (0)30 3087748- 0
Hegelplatz 1 info@ibu-epd.com
10117 Berlin www.ibu-epd.com
Germany
Author of the Life Cycle Assessment
brands & values GmbH +49 421 70 90 84 33
Hollerallee 14A info@brandsandvalues.com
28209 Bremen www.brandsandvalues.com
Germany
Owner of the Declaration
Hansgrohe Group +49 7836 51-0
Auestr. 5-9 info@hansgrohe-group.com
77761 Schiltach www.hansgrohe-group.com
Germany
10 Environmental Product Declaration - Hansgrohe Group - Toilets
