ENVIRONMENTAL PRODUCT DECLARATION
as per ISO 14025 and EN 15804+A2
Owner of the Declaration dormakaba International Holding GmbH
Publisher Institut Bauen und Umwelt e.V. (IBU)
Programme holder Institut Bauen und Umwelt e.V. (IBU)
Declaration number EPD-DOR-20230452-CBA2-EN
Issue date 27/11/2023
Valid to 26/11/2028
Crane Automatic Revolving Door - AL 1000/2000/3000
dormakaba
www.ibu-epd.com | https://epd-online.com
General Information
dormakaba Crane Automatic Revolving Door - AL
1000/2000/3000
Programme holder Owner of the declaration
IBU – Institut Bauen und Umwelt e.V. dormakaba International Holding GmbH
Hegelplatz 1 DORMA Platz 1
10117 Berlin 58256 Ennepetal
Germany Germany
Declaration number Declared product / declared unit
EPD-DOR-20230452-CBA2-EN 1 piece of the product: Automatic Revolving Door AL 1000/2000/3000, with
a diameter of 10 ft. (3050 mm) and a height of 7,5 ft. (2290 mm),
consisting of the following items:
• 4 door leaves
• Enclosure
• Canopy
• Product packaging
This declaration is based on the product category rules: Scope:
Automatic doors, automatic gates, and revolving door systems, This Environmental Product Declaration refers to a specific automatic
01/08/2021 revolving door manufactured by dormakaba. The production site is located
(PCR checked and approved by the SVR) in Reamstown (USA).
The data represents the year 2022.
Issue date The owner of the declaration shall be liable for the underlying information
and evidence; the IBU shall not be liable with respect to manufacturer
27/11/2023
information, life cycle assessment data and evidences.
The EPD was created according to the specifications of EN 15804+A2. In
Valid to
the following, the standard will be simplified as EN 15804.
26/11/2028
Verification
The standard EN 15804 serves as the core PCR
Independent verification of the declaration and data according to ISO
14025:2011
internally X externally
Dipl.-Ing. Hans Peters
(Chairman of Institut Bauen und Umwelt e.V.)
Florian Pronold Matthias Klingler,
(Managing Director Institut Bauen und Umwelt e.V.) (Independent verifier)
1 Environmental Product Declaration - dormakaba - Crane Automatic Revolving Door - AL 1000/2000/3000
Product
The product with respect to its characteristics are in accordance
Product description/Product definition with the relevant technical provisions (no CE-marking):
The Crane Automatic Revolving Door 1000/2000/3000 is
• ANSI 156.27
designed as a building's primary entrance. A range of available
• 2011/65/EU ROHS3 Directive
finishes allows the integration into its surrounding décor and
architecture. The technical and safety features ensure smooth
and safe traffic flow. The Crane 1000/2000/3000 doors feature Base materials/Ancillary materials
the same automatic drive system. The Crane 2000 and 3000
The major material composition including the packaging of the
series fullfill higher quality standards and are more customized.
product is listed below:
In these ways, the Crane revolving doors fulfill both aesthetic
Name Value Unit
and functional requirements.
Glass 59 %
For the Crane Automatic Revolving Door 1000/2000/3000 the Aluminium 31 %
standards which can be applied are the following: Electronics 5 %
• ANSI 156.27 Zinc 4 %
• 2011/65/EU ROHS3 Directive Plastics 1 %
The product includes partial articles which contain substances
Application listed in the Candidate List of REACH Regulation
Revolving doors may be used to provide a comfortable entry 1907/2006/EC (date: 14.06.2023) exceeding 0.1 percentage by
and exit in many applications in the facade of or within a mass: no
building. Typical applications include:
The Candidate List can be found on the ECHA website
• Hotels
address: https:echa.europa.eu/de/home.
• Healthcare settings
• Airports and transportation facilities Reference service life
• Commercial office buildings
The reference service life of the Crane Automatic Revolving
• Institutional and educational buildings
door AL 1000/2000/3000 amounts to 20 years, depending on
• Retail stores
the application and frequency of use. For repairs and renewals,
suitable spare parts are available. The revolving door is tested
Technical Data
and certified to ANSI 156.27, meaning they are designed to
The Crane Automatic Revolving Doors AL 1000/2000/3000
withstand a minimum of 1.000.000 cycles.
have following technical properties:
Name Value Unit
Height range 1000/2000 7-9 ft
Height range 3000 7+ ft
Diameter range maximum
12 ft
1000/2000/3000
clear or tinted
Enclosure glass 1000/2000 7/16"
laminated
clear or tinted
Enclosure glass 3000 9/16"
laminated
Door leaf glass 1/4" tempered
LCA: Calculation rules
treatments, processing of secondary material input (e.g.
Declared Unit recycling processes), — A2, transport to the manufacturer, —
A3, manufacturing and assembly including provision of all
The declared unit is 1 piece of the product: Automatic materials, products and energy, as well as waste processing up
Revolving Door AL 1000/2000/3000 to the end-of waste state.
Name Value Unit
Construction stage - Modules A4-A5
Declared unit 1 piece/product
The construction process stage includes:
Mass of declared Product 896 kg
— A4, transport to the building site; — A5, installation into the
building; including provision of all materials, products and
energy, as well as waste processing up to the end-of waste
System boundary
state or disposal of final residues during the construction
The type of EPD is: cradle to gate with options, modules C1– process stage.
C4, and module D (A1–A3 + C + D and additional modules:
A4+ A5+B6) Use stage - Module B6
The use stage related to the operation of the building
Production - Module A1-A3 includes: — B6, operational energy use.
The product stage includes:
— A1, raw material extraction, processing and mechanical End-of-life stage– Modules C1-C4 and D
2 Environmental Product Declaration - dormakaba - Crane Automatic Revolving Door - AL 1000/2000/3000
The end-of-life stage includes: manufactured, used or handled at the end of the product´s
— C1, de-construction, demolition: — C2, transport to waste lifespan: Global
processing; — C3, waste processing for reuse, recovery and/or
recycling; — C4, disposal; including provision and all transport,
Comparability
provision of all materials, products and related energy and
water use. Module D (Benefits and loads beyond the system Basically, a comparison or an evaluation of EPD data is only
boundary) includes: — D, recycling potentials, expressed as net possible if all the data sets to be compared were created
impacts and benefits. according to EN 15804 and the building context, respectively
the product-specific characteristics of performance, are taken
Geographic Representativeness into account. Background database: GaBi, SP40.
Land or region, in which the declared product system is
LCA: Scenarios and additional technical information
Name Value Unit
Characteristic product properties of biogenic carbon
Electricity consumption for 1 year 1964,5 kWh
Days per year in use 365 days
Information on describing the biogenic carbon content at
On mode per day 5 h
factury gate
Idle mode per day 19 h
Name ValueUnit
On mode power 300 W
kg
Biogenic carbon content in product - Idle mode power 200 W
C
Biogenic carbon content in accompanying - kg End of life (C1-C4)
packaging C
C1: The product expansion depends on the building. The
product share is so low that no environmental burden is
assumed.
C2: Transport to waste management is 50 km.
Transport to the building site (A4) Name Value Unit
Name Value Unit Collected separately waste type waste type 887 kg
Litres of fuel 0.00276 l/100km Recycling 318 kg
Transport distance 50 km Energy recovery 3.08 kg
Capacity utilisation (including empty runs) 55 % Landfilling 565 kg
The product is transported via truck. The main distribution The product is disassembled in a recycling process. Material
region is North America. In order to allow scaling to a specific recycling is then assumed for metals and electronics. The
point of installation 100 km is declared. plastic components are assumed to be incinerated with energy
recovery. Minor proportions of residues arising from the
recycling process are landfilled. Region for the End of Life is:
Installation into the building (A5)
Global.
Name Value Unit
Waste packaging (paper and plastic) 8 kg Reuse, recovery and/or recycling potentials (D), relevant
scenario information
Reference service life Name Value Unit
Recycling 100 %
Name Value Unit
Life Span according to the manufacturer 20 a The collection rate is 100 %.
Operational energy use (B6)
3 Environmental Product Declaration - dormakaba - Crane Automatic Revolving Door - AL 1000/2000/3000
LCA: Results
DESCRIPTION OF THE SYSTEM BOUNDARY (X = INCLUDED IN LCA; MND = MODULE OR INDICATOR NOT DECLARED; MNR
= MODULE NOT RELEVANT)
Benefits and
Construction loads beyond
Product stage Use stage End of life stage
process stage the system
boundaries
la ire ta m w a Ry lp p u s tro p s n a rT g n iru tc a fu n a M e h t m o rf tro p s n a rTe tis e h t o t e ta g y lb m e s s A e s U e c n a n e tn ia M ria p e R tn e m e c a lp e R tn e m h s ib ru fe R y g re n e la n o ita re p Oe s u re ta w la n o ita re p Oe s u n o itc u rts n o c -e Dn o itilo m e d tro p s n a rT g n is s e c o rp e ts a W la s o p s iD -e s u e R-y re v o c e R-g n ilc y c e Rla itn e to p
A1 A2 A3 A4 A5 B1 B2 B3 B4 B5 B6 B7 C1 C2 C3 C4 D
X X X X X MND MND MNR MNR MNR X MND X X X X X
RESULTS OF THE LCA - ENVIRONMENTAL IMPACT according to EN 15804+A2: 1 piece AL 1000/2000/3000
Parameter Unit A1-A3 A4 A5 B6 C1 C2 C3 C4 D
GWP-total kg CO 2 eq 4.53E+03 7.83E+00 2.29E+01 2.21E+04 0 3.88E+00 7.83E+00 8.63E+00 -1.78E+03
GWP-fossil kg CO 2 eq 4.52E+03 7.49E+00 2.29E+01 2.21E+04 0 3.71E+00 7.83E+00 8.57E+00 -1.77E+03
GWP-biogenic kg CO 2 eq 7.04E+00 3.46E-01 5.33E-04 4.78E+00 0 1.71E-01 1.82E-04 2.9E-02 -5.77E+00
GWP-luluc kg CO 2 eq 1.78E+00 1.78E-04 1E-03 6.65E+00 0 8.82E-05 4.43E-04 2.5E-02 -3.22E-01
ODP kg CFC11 eq 2.95E-11 7.9E-16 1.15E-14 7.77E-11 0 3.91E-16 3.95E-15 3.18E-14 -1.38E-08
AP mol H+ eq 2.14E+01 7E-03 4E-03 3.57E+01 0 4E-03 1E-03 6.2E-02 -6.94E+00
EP-freshwater kg P eq 3.49E-03 1.6E-06 1.84E-06 1.2E-02 0 7.93E-07 6.3E-07 1.47E-05 -1E-03
EP-marine kg N eq 3.6E+00 2E-03 9.18E-04 7.64E+00 0 1E-03 3.14E-04 1.6E-02 -9.02E-01
EP-terrestrial mol N eq 4E+01 2.7E-02 1.9E-02 8.2E+01 0 1.3E-02 6E-03 1.74E-01 -9.79E+00
kg NMVOC
POCP 9.53E+00 7E-03 3E-03 2.18E+01 0 3E-03 8.7E-04 4.8E-02 -2.88E+00
eq
ADPE kg Sb eq 1.64E-01 2.25E-07 1.58E-07 4E-03 0 1.11E-07 5.42E-08 7.7E-07 -5.3E-02
ADPF MJ 6.18E+04 1.06E+02 1.06E+01 3.57E+05 0 5.26E+01 3.63E+00 1.12E+02 -2.54E+04
m3 world eq
WDP 6.56E+02 1.5E-02 2.34E+00 4.27E+03 0 7E-03 8.01E-01 8.99E-01 -9.62E+01
deprived
GWP = Global warming potential; ODP = Depletion potential of the stratospheric ozone layer; AP = Acidification potential of land and water; EP =
Eutrophication potential; POCP = Formation potential of tropospheric ozone photochemical oxidants; ADPE = Abiotic depletion potential for non-fossil
resources; ADPF = Abiotic depletion potential for fossil resources; WDP = Water (user) deprivation potential)
RESULTS OF THE LCA - INDICATORS TO DESCRIBE RESOURCE USE according to EN 15804+A2: 1 piece AL 1000/2000/3000
Parameter Unit A1-A3 A4 A5 B6 C1 C2 C3 C4 D
PERE MJ 1.79E+04 3.35E-01 2.76E+00 5.65E+04 0 1.66E-01 9.44E-01 1.47E+01 -1.2E+04
PERM MJ 0 0 0 0 0 0 0 0 0
PERT MJ 1.79E+04 3.35E-01 2.76E+00 5.65E+04 0 1.66E-01 9.44E-01 1.47E+01 -1.2E+04
PENRE MJ 6.14E+04 1.06E+02 3.98E+02 3.57E+05 0 5.26E+01 1.15E+02 1.13E+02 -2.54E+04
PENRM MJ 4.98E+02 0 -3.87E+02 0 0 0 -1.11E+02 0 0
PENRT MJ 6.19E+04 1.06E+02 1.06E+01 3.57E+05 0 5.26E+01 3.63E+00 1.13E+02 -2.54E+04
SM kg 1.95E+00 0 0 0 0 0 0 0 0
RSF MJ 0 0 0 0 0 0 0 0 0
NRSF MJ 0 0 0 0 0 0 0 0 0
FW m3 4.29E+01 6.01E-04 5.6E-02 1.31E+02 0 2.97E-04 1.9E-02 2.8E-02 -2.1E+01
PERE = Use of renewable primary energy excluding renewable primary energy resources used as raw materials; PERM = Use of renewable primary
energy resources used as raw materials; PERT = Total use of renewable primary energy resources; PENRE = Use of non-renewable primary energy
excluding non-renewable primary energy resources used as raw materials; PENRM = Use of non-renewable primary energy resources used as raw
materials; PENRT = Total use of non-renewable primary energy resources; SM = Use of secondary material; RSF = Use of renewable secondary fuels;
NRSF = Use of non-renewable secondary fuels; FW = Use of net fresh water
RESULTS OF THE LCA – WASTE CATEGORIES AND OUTPUT FLOWS according to EN 15804+A2:
1 piece AL 1000/2000/3000
Parameter Unit A1-A3 A4 A5 B6 C1 C2 C3 C4 D
HWD kg 3.99E-05 1.03E-08 4.04E-08 1.38E-04 0 5.1E-09 1.38E-08 1.72E-06 -5.89E-05
NHWD kg 8.29E+02 1.1E-02 2.38E+00 1.11E+02 0 5E-03 8.13E-01 5.66E+02 -4.55E+02
RWD kg 3.58E+00 1.14E-04 3.94E-04 3.18E+01 0 5.65E-05 1.35E-04 1E-03 -2.84E+00
CRU kg 0 0 0 0 0 0 0 0 0
MFR kg 0 0 0 0 0 0 3.18E+02 0 0
MER kg 0 0 0 0 0 0 0 0 0
EEE MJ 0 0 4.24E+01 0 0 0 1.45E+01 0 0
EET MJ 0 0 9.73E+01 0 0 0 3.33E+01 0 0
4 Environmental Product Declaration - dormakaba - Crane Automatic Revolving Door - AL 1000/2000/3000
HWD = Hazardous waste disposed; NHWD = Non-hazardous waste disposed; RWD = Radioactive waste disposed; CRU = Components for re-use;
MFR = Materials for recycling; MER = Materials for energy recovery; EEE = Exported electrical energy; EET = Exported thermal energy
RESULTS OF THE LCA – additional impact categories according to EN 15804+A2-optional:
1 piece AL 1000/2000/3000
Parameter Unit A1-A3 A4 A5 B6 C1 C2 C3 C4 D
Disease
PM 1.89E-04 3.94E-08 5.2E-08 3.19E-04 0 1.95E-08 1.78E-08 7.61E-07 -1.11E-04
incidence
IR kBq U235 eq 5.54E+02 1.6E-02 3.5E-02 2.63E+03 0 8E-03 1.2E-02 1.32E-01 -5.69E+02
ETP-fw CTUe 3.45E+04 7.53E+01 3.98E+00 1.06E+05 0 3.73E+01 1.36E+00 6.43E+01 -9.85E+03
HTP-c CTUh 1.88E-06 1.42E-09 3.45E-10 2.29E-06 0 7.01E-10 1.18E-10 9.52E-09 6.25E-08
HTP-nc CTUh 6.02E-05 6.06E-08 3.49E-08 8.66E-05 0 3E-08 1.19E-08 1.05E-06 4.7E-05
SQP SQP 5.11E+03 2.73E-01 3.18E+00 3.27E+04 0 1.35E-01 1.09E+00 2.35E+01 -7.43E+02
PM = Potential incidence of disease due to PM emissions; IR = Potential Human exposure efficiency relative to U235; ETP-fw = Potential comparative
Toxic Unit for ecosystems; HTP-c = Potential comparative Toxic Unit for humans (cancerogenic); HTP-nc = Potential comparative Toxic Unit for humans
(not cancerogenic); SQP = Potential soil quality index
Disclaimer 1 – for the indicator “Potential Human exposure efficiency relative to U235”. This impact category deals mainly with the
eventual impact of low-dose ionizing radiation on human health of the nuclear fuel cycle. It does not consider effects due to possible
nuclear accidents, occupational exposure or radioactive waste disposal in underground facilities. Potential ionizing radiation from the
soil, radon and from some construction materials is also not measured by this indicator.
Disclaimer 2 – for the indicators “abiotic depletion potential for non-fossil resources”, “abiotic depletion potential for fossil resources”,
“water (user) deprivation potential, deprivation-weighted water consumption”, “potential comparative toxic unit for ecosystems”,
“potential comparative toxic unit for humans – cancerogenic”, “Potential comparative toxic unit for humans - not cancerogenic”,
“potential soil quality index”. The results of this environmental impact indicator shall be used with care as the uncertainties on these
results are high as there is limited experience with the indicator.
This EPD was created using a software tool.
References
ANSI 156.27 e.V., 2021. www.ibu-epd.com
ANSI/BHMA A156.27-2019, Power and Manual Operated
Revolving Pedestrian Doors GaBi
Sphera Solutions GmbH Gabi Software System and Database
EN 15804 for Life Cycle Engineering 19922020 Version 10.0.0.71
EN 15804+A2:2019+AC:2021, Sustainability of construction University of Stuttgart Leinfelden-Echterdingen
works — Environmental Product Declarations — Core rules for
the product category of construction products GaBi ts documentation
GaBi life cycle inventory data documentation
ISO 14025 (https://www.gabisoftware.com/support/gabi/gabidatabase-
DIN EN ISO 14025:201110, Environmental labels and 2020-lcidocumentation/).
declarations — Type III environmental declarations —
Principles and procedures LCA-tool dormakaba
Tool No.: IBU-DOR-202107-LT1-EN .
REACH Developed by Sphera Solutions GmbH
Regulation (EC) No 1907/2006 of the European Parliament and
of the Council on the Registration, Evaluation, Authorisation PCR Part A
and Restriction of Chemicals (REACH) PCR – Part A: Calculation Rules for the Life Cycle Assessment
and Requirements on the Project Re-port according to EN
2011/65/EU ROHS3 Directive 15804+A2:2019, Version 1.0, 2020, Institut Bauen und Umwelt
Directive 2011/65/EU of the European Parliament and of the e.V.,
Council of 8 June 2011 on the restriction of the use of certain www.ibu-epd.com.
hazardous substances in electrical and electronic equipment
PCR Part B
Further References PCR – Part B: Requirements on the EPD for Automatic doors,
automatic gates, and revolving door systems, version 6, Institut
IBU 2021 Bauen und Umwelt e.V.,
General Instructions for the EPD programme of Institut Bauen www.ibu-epd.com.
und Umwelt e.V. Version 2.0, Berlin: Institut Bauen und Umwelt
5 Environmental Product Declaration - dormakaba - Crane Automatic Revolving Door - AL 1000/2000/3000
Publisher
Institut Bauen und Umwelt e.V. +49 (0)30 3087748- 0
Hegelplatz 1 info@ibu-epd.com
10117 Berlin www.ibu-epd.com
Germany
Programme holder
Institut Bauen und Umwelt e.V. +49 (0)30 3087748- 0
Hegelplatz 1 info@ibu-epd.com
10117 Berlin www.ibu-epd.com
Germany
Author of the Life Cycle Assessment
dormakaba International Holding GmbH +49 2333 793-0
DORMA Platz 1 info.de@dormakaba.com
58256 Ennepetal www.dormakaba.com
Germany
Owner of the Declaration
dormakaba International Holding GmbH +49 2333 793-0
DORMA Platz 1 info.de@dormakaba.com
58256 Ennepetal www.dormakaba.com
Germany
6 Environmental Product Declaration - dormakaba - Crane Automatic Revolving Door - AL 1000/2000/3000
