ENVIRONMENTAL PRODUCT DECLARATION
as per ISO 14025 and EN 15804+A2
Owner of the Declaration Milliken Industrials Ltd.
Programme holder Institut Bauen und Umwelt e.V. (IBU)
Publisher Institut Bauen und Umwelt e.V. (IBU)
Declaration number EPD-MIL-20220313-CBA1-EN
Issue date 09.01.2023
Valid to 08.01.2028
Luxury Vinyl Tiles (LVT) FlexForm™/FlexForm™ Sound
Milliken
www.ibu-epd.com | https://epd-online.com
Umwelt Produktdeklaration Name des Herstellers – Name des Produkts
General Information
Milliken Luxury Vinyl Tiles (LVT)
FlexForm™/FlexForm™ Sound
Programme holder Owner of the declaration
IBU – Institut Bauen und Umwelt e.V. Milliken Industrials Ltd.
Hegelplatz 1 Beech Hill Plant, Gidlow Lane
10117 Berlin Wigan WN6 8RN
Germany United Kingdom
Declaration number Declared product / declared unit
EPD-MIL-20220313-CBA1-EN 1 m² Luxury Vinyl Tiles FlexForm™/FlexForm™
Sound.
This declaration is based on the product Scope:
category rules: The manufacturer declaration applies to Luxury Vinyl
Floor coverings, 07.2022 Tile (LVT) FlexForm™/FlexForm™ Sound.
(PCR checked and approved by the SVR) The carpet is manufactured in South Korea.
Issue date The owner of the declaration shall be liable for the
09.01.2023 underlying information and evidence; the IBU shall not
be liable with respect to manufacturer information, life
Valid to cycle assessment data and evidences.
08.01.2028 The EPD was created according to the specifications
of EN 15804+A2. In the following, the standard will be
simplified as EN 15804.
Verification
The standard EN 15804 serves as the core PCR
Independent verification of the declaration and data
according to ISO 14025:2011
Dipl. Ing. Hans Peters internally x externally
(chairman of Institut Bauen und Umwelt e.V.)
Dr. Alexander Röder Angela Schindler
(Managing Director Institut Bauen und Umwelt e.V.)) (Independent verifier)
Product
Product description/Product definition
Luxury Vinyl Tile (LVT) FlexformTM Sound
2 Environmental Product Declaration Milliken – Luxury Vinyl Tiles (LVT) FlexForm™/FlexForm™ Sound
Multilayer vinyl tile, type 1, with an overall thickness of
5 mm and a total weight of 7600 g/m2 for FlexForm™
and 8000 g/m2 for FlexForm™ Sound. FlexForm™ Performance data of the product in accordance with
Sound has the same construction as FlexForm™ but the declaration of performance with respect to its
with a Sound Compact Cushion Layer. essential characteristics according to EN 14041:
The LCA results are calculated with the weight of the 2018-05, Resilient, textile and laminate floor coverings
heaviest product. - Essential characteristics.
For the placing on the market of the product in the Additional product properties in accordance with ISO
European Union/European Free Trade Association 10582 can be found on the manufacturer's technical
(EU/EFTA) (with the exception of Switzerland) information section (www.millikencarpet.com).
Regulation (EU) No. 305/2011 Construction Product
Regulation (CPR) applies. The product needs a Base materials/Ancillary materials
Declaration of Performance (DoP) taking into
consideration EN 14041-2018-05, Resilient, textile and Name Value Unit
laminate floor coverings - Essential characteristics and Limestone 61.3 %
the CE-marking. The DoP of the product can be found Polyvinyl chloride 25.0 %
on the manufacturer's technical information section. Plasticizer 12.2 %
For the application and use of the product the Glass fibre 0.6 %
respective national provisions apply. Stabilizer 0.4 %
Polyurethane 0.3 %
Application Pigments 0.2 %
According to the use class as defined in ISO 10582 the
This product contains substances listed in the ECHA
product can be used in all professional areas with
candidate list (10.06.2022) or other carcinogenic,
heavy use which require class 33 and in all industrial
mutagenic or reprotoxic (CMR) substances in
areas with general use which require class 42.
categories 1A or 1B which are not on the ECHA
candidate list exceeding 0.1 percentage by mass: no
Reference service life
The service life of resilient floor coverings strongly
Technical Data depends on the correct installation taking into account
The performance data listed in the DoP apply. the declared use classification and the adherence to
cleaning and maintenance instructions.
Constructional data A calculation of the reference service life according to
Name Value Unit ISO 15686 is not possible.
Product thickness 5 mm Alternatively, a reference service life of 20 years can
Thickness of the wear be assumed, during which the functional and visual
0.55 mm
layer quality is guaranteed (BNB, Nutzungsdauer von
FlexForm™ 7600 Bauteilen). The technical service life can be
Grammage g/m2
FlexForm™ Sound 8000 significantly longer.
Product Form Tiles 250 mm x 1500 mm -
Type of manufacture Multilayer vinyl tile, type 1 -
ProGuard MAXᵀᴹ
Finish
UV-cured urethane
Edge profile Micro bevel
LCA: Calculation rules
Declared Unit 1 - landfill disposal
2 - municipal waste incineration
Name Value Unit A1-A3 Production:
Declared unit 1 m2 Energy supply and production of the basic material,
Grammage FlexForm™ 7.6 kg/m² processing of secondary material, auxiliary material,
Grammage FlexForm™ Sound 8 kg/m2 transport of the material to the manufacturing site,
Layer thickness 0.005 m emissions, waste water treatment, packaging material
Gross density FlexForm™ 1520 kg/m³ and waste processing up to the landfill disposal of
Gross density FlexForm™ Sound 1600 kg/m3 residual waste (except radioactive waste). Benefits for
The declared unit refers to 1 m2 produced resilient floor generated electricity and steam due to the incineration
covering. The output of module A5 'Assembly' is 1 m2 of production waste are aggregated.
installed resilient floor covering. Biogenic carbon that is stored in renewable material
(packaging paper and wooden pallets) is taken into
account as well as the associated carbon dioxide
System boundary uptake from the air from which this biogenic carbon
Type of EPD originates.
Cradle-to-gate with options, module C1-C4, module D,
and additional modules A4, A5, B1, B2 A4 Transport:
System boundaries of modules A, B, C, D Modules C3, Transport of the packed resilient floor covering from
C4 and D are indicated separately for two end-of-life the Milliken factory gate to the place of installation.
scenarios:
3 Environmental Product Declaration Milliken – Luxury Vinyl Tiles (LVT) FlexForm™/FlexForm™ Sound
A5 Installation:
Installation of the resilient floor covering, processing of C1 De-construction:
installation waste and packaging waste up to the The floor covering is de-constructed manually and no
landfill disposal of residual waste (except radioactive environmental impact is caused.
waste), the production of the amount of floor covering
that occurs as installation waste including its transport C2 Transport:
to the place of installation. Transport of the floor-covering waste to a landfill or to
Generated electricity and steam due to the incineration the municipal waste incineration plant (MWI)
of waste are listed in the result table as exported
energy. C3 Waste processing:
Biogenic carbon that is stored in renewable materials C3-1: Landfill disposal needs no waste processing.
(wooden pallets and packaging paper) is released as C3-2: The impact from waste incineration (plant with
carbon dioxide emissions into the air at the end of life R1>0.6), generated electricity and steam are listed in
in module A5. the result table as exported energy.
Preparation of the floor and auxiliary materials (fixing
agents for the edges) are beyond the system C4 Disposal
boundaries and not taken into account. C4-1: Impact from landfill disposal.
C4-2: The carpet waste leaves the system in
B1 Use: module C3-2.
Indoor emissions during the use stage are very low
(certificate Indoor Air Comfort Gold) and not taken into D Recycling potential:
account. D-A5: Benefits for generated energy due
to incineration of packaging and installation waste
B2 Maintenance: (incineration plant with R1 > 0.6),
Cleaning of the resilient floor covering for a period of 1 D-1: There are no benefits for generated energy due to
year: landfill disposal of plastic waste at the end-of-life,
Dry mopping (without environmental impacts), D-2: Benefits for generated energy due to incineration
damp mopping – water consumption, production of the of floor covering waste at the end-of-life (incineration
cleaning agent, waste water treatment. plant with R1 > 0.6),
The declared values in this module have to be
multiplied by the assumed service life of the floor Comparability
covering in the building in question. Basically, a comparison or an evaluation of EPD data
is only possible if all the data sets to be compared
B3 - B5 Repair, replacement, refurbishment were created according to EN 15804 and the building
The modules are not relevant within the assumed context, respectively the product-specific
reference service life of 20 years. characteristics of performance, are taken into account.
B6 - B7 Operational energy and water use Background data are taken from the GaBi database
No energy and water input are required for the 2021-2. Remaining data gaps are covered by the
operation of the resilient floor covering in the use ecoinvent 3.7 database 2020.
stage. The modules are not relevant and not declared
LCA: Scenarios and additional technical information
Characteristic product properties Maintenance (B2)
Information on biogenic carbon The values for cleaning refer to 1 m2 floor covering per
year. Depending on the application based on ISO
10874, the technical service life recommended by the
Information on describing the biogenic Carbon manufacturer and the anticipated strain on the floor by
Content at factory gate customers, the case-specific useful life can be
Name Value Unit established. Based on this useful life the effects of
Biogenic carbon content in Module B2 need to be calculated in order to obtain the
0.107 kg C
accompanying packaging overall environmental impacts.
1 kg biogenic Carbon is equivalent to 44/12 kg of CO Name Value Unit
2
Maintenance cycle (dry mopping) 208 1/year
Maintenance cycle (damp mopping) 52 1/year
Water consumption (damp mopping) 0.0013 m3
Transport to the construction site (A4) Cleaning agent (damp mopping) 0.0042 kg
Name Value Unit For further information on cleaning and maintenance
Litres of fuel 0.02 l/100km see www.millikencarpet.com
Transport distance 700 km
Capacity utilisation (including empty
55 %
runs)
Gross density of products transported 1600 kg/m3
Installation in the building (A5)
Name Value Unit
Material loss 0.24 kg
4 Environmental Product Declaration Milliken – Luxury Vinyl Tiles (LVT) FlexForm™/FlexForm™ Sound
Reference service life
Name Value Unit
Life Span (according to
20 a
BBSR)
Corresponds to the
Declared product properties
specifications of ISO -
(at the gate) and finishes
10582
An assumed quality of
Conforms to the
work, when installed in
manufacturer's -
accordance with the
instructions
manufacturer’s instructions
Use in areas
Usage conditions, e.g. corresponding to use
frequency of use, class 33 or 42 -
mechanical exposure according to ISO
10582
Maintenance e.g. required
According to the
frequency, type and quality
manufacturers -
and replacement of
instructions
components
End of Life (C1-C4)
Two different end-of-life scenarios are declared and
the results are indicated separately in module C.
Each scenario is calculated as a 100% scenario.
Scenario 1: 100 % landfill disposal
Scenario 2: 100 % municipal waste incineration (MWI)
with R1>0.6
If combinations of these scenarios have to be
calculated this should be done according to the
following scheme:
EOL-impact = x % impact (Scenario 1)
+ y % impact (Scenario 2)
with x % + y % = 100 %
Name Value Unit
Collected as mixed construction
8 kg
waste (scenarios 1 and 2)
Landfilling (scenario 1) 8 kg
Energy recovery (scenario 2) 8 kg
Reuse, recovery and/or recycling potentials (D),
relevant scenario information
Recovery potentials due to the two end-of-life
scenarios (module C) are indicated separately.
5 Environmental Product Declaration Milliken – Luxury Vinyl Tiles (LVT) FlexForm™/FlexForm™ Sound
LCA: Results
The modules C3/1 and C4/2 cause no additional impact (see chapter "LCA: Calculation rules"). Module C2
represents the transport for scenarios 1 and 2. The values in column D result from module A5.
DESCRIPTION OF THE SYSTEM BOUNDARY (X = INCLUDED IN LCA; ND = MODULE OR INDICATOR NOT
DECLARED; MNR = MODULE NOT RELEVANT)
BENEFITS AND
CONSTRUCTI LOADS
PRODUCT STAGE ON PROCESS USE STAGE END OF LIFE STAGE BEYOND THE
STAGE SYSTEM
BOUNDARIES
6 Environmental Product Declaration Milliken – Luxury Vinyl Tiles (LVT) FlexForm™/FlexForm™ Sound
lairetam
waR
ylppus tropsnarT
gnirutcafunaM
eht
morf
tropsnarT
etis
eht
ot
etag
ylbmessA esU
ecnanetniaM
riapeR
tnemecalpeR tnemhsibrufeR
ygrene
lanoitarepO esu
retaw
lanoitarepO esu
noitcurtsnoc-eD
noitilomed tropsnarT
gnissecorp
etsaW
lasopsiD -esueR -yrevoceR -gnilcyceR laitnetop
A1 A2 A3 A4 A5 B1 B2 B3 B4 B5 B6 B7 C1 C2 C3 C4 D
X X X X X X X MNR MNR MNR ND ND X X X X X
RESULTS OF THE LCA - ENVIRONMENTAL IMPACT according to EN 15804+A2: 1 m² resilient floor
covering
Core Indicator Unit A1-A3 A4 A5 B1 B2 C1 C2 C3/2 C3/3 C4/1 D D/1 D/2 D/3
-
GWP-total [kg CO2-Eq.] 1.06E+15.25E-11.01E+00.00E+01.24E-20.00E+02.91E-29.51E+00.00E+06.02E-1-3.91E-20.00E+0 1.30E+00.00E+0
-
GWP-fossil [kg CO2-Eq.] 1.09E+15.15E-1 6.30E-10.00E+01.21E-20.00E+02.86E-29.51E+00.00E+06.01E-1-3.89E-20.00E+0 1.30E+00.00E+0
GWP-biogenic [kg CO2-Eq.] -3.52E-16.67E-3 3.81E-10.00E+02.85E-40.00E+03.70E-4 1.66E-30.00E+07.27E-8-1.91E-40.00E+0-6.35E-30.00E+0
GWP-luluc [kg CO2-Eq.] 6.37E-3 2.92E-3 3.15E-40.00E+07.63E-60.00E+01.62E-4 9.58E-40.00E+02.96E-4-4.06E-60.00E+0-1.35E-40.00E+0
6.50E- 3.13E- 1.97E- 1.70E- 1.74E- 5.57E- 8.16E- -2.46E- -8.20E-
ODP [kg CFC11-Eq.] 0.00E+0 0.00E+0 0.00E+0 0.00E+0 0.00E+0
10 14 11 15 15 12 13 13 12
AP [mol H+-Eq.] 7.71E-2 3.11E-3 2.51E-30.00E+01.56E-50.00E+01.73E-4 3.20E-30.00E+01.80E-3-4.93E-50.00E+0-1.64E-30.00E+0
EP-freshwater [kg P-Eq.] 1.96E-5 1.56E-6 7.31E-70.00E+02.60E-70.00E+08.66E-8 3.07E-60.00E+01.13E-4-5.02E-80.00E+0-1.67E-60.00E+0
EP-marine [kg N-Eq.] 2.15E-2 1.53E-3 7.29E-40.00E+05.62E-60.00E+08.48E-5 1.19E-30.00E+03.99E-4-1.36E-50.00E+0-4.53E-40.00E+0
EP-terrestrial [mol N-Eq.] 2.35E-1 1.69E-2 8.00E-30.00E+05.01E-50.00E+09.39E-4 1.37E-20.00E+04.37E-3-1.46E-40.00E+0-4.86E-30.00E+0
POCP [kg NMVOC-Eq.]7.17E-2 2.89E-3 2.34E-30.00E+03.50E-50.00E+01.60E-4 3.25E-30.00E+01.28E-3-3.82E-50.00E+0-1.27E-30.00E+0
ADPE [kg Sb-Eq.] 6.77E-5 4.37E-8 2.04E-60.00E+01.80E-80.00E+02.43E-9 1.69E-70.00E+04.22E-8-5.61E-90.00E+0-1.87E-70.00E+0
-
ADPF [MJ] 2.41E+26.99E+07.88E+00.00E+03.11E-10.00E+03.88E-11.40E+10.00E+08.62E+0-6.60E-10.00E+0 0.00E+0
2.20E+1
[m³ world-Eq
WDP 6.15E-1 4.68E-3 5.53E-20.00E+04.36E-20.00E+02.60E-41.23E+00.00E+0-6.45E-3-3.83E-30.00E+0-1.28E-10.00E+0
deprived]
GWP = Global warming potential; ODP = Depletion potential of the stratospheric ozone layer; AP = Acidification potential of land and water; EP =
Caption Eutrophication potential; POCP = Formation potential of tropospheric ozone photochemical oxidants; ADPE = Abiotic depletion potential for non-
fossil resources; ADPF = Abiotic depletion potential for fossil resources; WDP = Water (user) deprivation potential
RESULTS OF THE LCA - INDICATORS TO DESCRIBE RESOURCE USE according to EN 15804+A2: 1 m²
resilient floor covering
Indicator Unit A1-A3 A4 A5 B1 B2 C1 C2 C3/2 C3/3 C4/1 D D/1 D/2 D/3
PERE [MJ] 2.12E+1 3.97E-1 4.04E+0 0.00E+0 2.33E-2 0.00E+0 2.21E-2 3.40E+0 0.00E+0 7.09E-1 -1.70E-1 0.00E+0 -5.67E+0 0.00E+0
PERM [MJ] 3.19E+0 0.00E+0 -3.19E+0 0.00E+0 0.00E+0 0.00E+0 0.00E+0 0.00E+0 0.00E+0 0.00E+0 0.00E+0 0.00E+0 0.00E+0 0.00E+0
PERT [MJ] 2.44E+1 3.97E-1 8.47E-1 0.00E+0 2.33E-2 0.00E+0 2.21E-2 3.40E+0 0.00E+0 7.09E-1 -1.70E-1 0.00E+0 -5.67E+0 0.00E+0
PENRE [MJ] 1.67E+2 7.01E+0 7.88E+0 0.00E+0 3.11E-1 0.00E+0 3.89E-1 8.77E+1 7.37E+1 8.63E+0 -6.60E-1 0.00E+0 -2.20E+1 0.00E+0
PENRM [MJ] 7.37E+1 0.00E+0 0.00E+0 0.00E+0 0.00E+0 0.00E+0 0.00E+0 -7.37E+1-7.37E+1 0.00E+0 0.00E+0 0.00E+0 0.00E+0 0.00E+0
PENRT [MJ] 2.41E+2 7.01E+0 7.88E+0 0.00E+0 3.11E-1 0.00E+0 3.89E-1 1.40E+1 0.00E+0 8.63E+0 -6.60E-1 0.00E+0 -2.20E+1 0.00E+0
SM [kg] 7.78E-2 0.00E+0 2.33E-3 0.00E+0 0.00E+0 0.00E+0 0.00E+0 0.00E+0 0.00E+0 0.00E+0 0.00E+0 0.00E+0 0.00E+0 0.00E+0
RSF [MJ] 0.00E+0 0.00E+0 0.00E+0 0.00E+0 0.00E+0 0.00E+0 0.00E+0 0.00E+0 0.00E+0 0.00E+0 0.00E+0 0.00E+0 0.00E+0 0.00E+0
NRSF [MJ] 0.00E+0 0.00E+0 0.00E+0 0.00E+0 0.00E+0 0.00E+0 0.00E+0 0.00E+0 0.00E+0 0.00E+0 0.00E+0 0.00E+0 0.00E+0 0.00E+0
FW [m³] 4.36E-2 4.49E-4 2.23E-3 0.00E+0 1.06E-3 0.00E+0 2.49E-5 3.01E-2 0.00E+0 1.01E-4 -1.63E-4 0.00E+0 -5.42E-3 0.00E+0
PERE = Use of renewable primary energy excluding renewable primary energy resources used as raw materials; PERM = Use of
renewable primary energy resources used as raw materials; PERT = Total use of renewable primary energy resources; PENRE = Use of
non-renewable primary energy excluding non-renewable primary energy resources used as raw materials; PENRM = Use of non-
Caption
renewable primary energy resources used as raw materials; PENRT = Total use of non-renewable primary energy resources; SM = Use
of secondary material; RSF = Use of renewable secondary fuels; NRSF = Use of non-renewable secondary fuels; FW = Use of net fresh
water
RESULTS OF THE LCA – WASTE CATEGORIES AND OUTPUT FLOWS according to EN 15804+A2:
1 m² resilient floor covering
Indicator Unit A1-A3 A4 A5 B1 B2 C1 C2 C3/2 C3/3 C4/1 D D/1 D/2 D/3
HWD [kg] 2.42E-6 3.36E-11 7.26E-8 0.00E+0 5.93E-11 0.00E+0 1.86E-12 1.36E-9 0.00E+0 1.33E-9 -9.13E-110.00E+0 -3.04E-9 0.00E+0
NHWD [kg] 1.62E-1 1.00E-3 1.85E-1 0.00E+0 7.58E-4 0.00E+0 5.57E-5 5.99E+0 0.00E+0 8.54E+0 -3.23E-4 0.00E+0 -1.08E-2 0.00E+0
RWD [kg] 3.88E-3 8.63E-6 1.31E-4 0.00E+0 3.06E-6 0.00E+0 4.79E-7 4.79E-4 0.00E+0 1.06E-4 -4.87E-5 0.00E+0 -1.62E-3 0.00E+0
CRU [kg] 0.00E+0 0.00E+0 0.00E+0 0.00E+0 0.00E+0 0.00E+0 0.00E+0 0.00E+0 0.00E+0 0.00E+0 0.00E+0 0.00E+0 0.00E+0 0.00E+0
MFR [kg] 0.00E+0 0.00E+0 8.90E-2 0.00E+0 0.00E+0 0.00E+0 0.00E+0 0.00E+0 0.00E+0 0.00E+0 0.00E+0 0.00E+0 0.00E+0 0.00E+0
MER [kg] 0.00E+0 0.00E+0 0.00E+0 0.00E+0 0.00E+0 0.00E+0 0.00E+0 0.00E+0 0.00E+0 0.00E+0 0.00E+0 0.00E+0 0.00E+0 0.00E+0
EEE [MJ] 0.00E+0 0.00E+0 1.63E-1 0.00E+0 0.00E+0 0.00E+0 0.00E+0 5.45E+0 0.00E+0 0.00E+0 0.00E+0 0.00E+0 0.00E+0 0.00E+0
EET [MJ] 0.00E+0 0.00E+0 3.33E-1 0.00E+0 0.00E+0 0.00E+0 0.00E+0 1.11E+1 0.00E+0 0.00E+0 0.00E+0 0.00E+0 0.00E+0 0.00E+0
HWD = Hazardous waste disposed; NHWD = Non-hazardous waste disposed; RWD = Radioactive waste disposed; CRU = Components
Caption for re-use; MFR = Materials for recycling; MER = Materials for energy recovery; EEE = Exported electrical energy; EET = Exported
thermal energy
RESULTS OF THE LCA – additional impact categories according to EN 15804+A2-optional:
1 m² resilient floor covering
Indicator Unit A1-A3 A4 A5 B1 B2 C1 C2 C3/2 C3/3 C4/1 D D/1 D/2 D/3
[Disease -4.08E-
PM 1.27E-6 1.80E-8 4.06E-8 0.00E+01.25E-100.00E+09.98E-10 6.48E-8 0.00E+0 1.73E-8 0.00E+0 0.00E+0 0.00E+0
Incidence] 10
[kBq U235-
IRP 4.39E-1 1.26E-3 1.50E-2 0.00E+0 3.08E-4 0.00E+0 7.02E-5 5.95E-2 0.00E+0 1.56E-2 -8.25E-3 0.00E+0 0.00E+0 0.00E+0
Eq.]
ETP-fw [CTUe] 1.05E+2 4.85E+0 3.64E+0 0.00E+0 1.38E-1 0.00E+0 2.69E-1 1.10E+1 0.00E+0 8.44E+0 -1.36E-1 0.00E+0 0.00E+0 0.00E+0
-6.55E-
HTP-c [CTUh] 3.79E-9 9.81E-111.30E-100.00E+04.44E-120.00E+05.44E-124.40E-100.00E+03.79E-10 0.00E+0 0.00E+0 0.00E+0
12
-2.53E-
HTP-nc [CTUh] 1.93E-7 5.82E-9 7.31E-9 0.00E+03.00E-100.00E+03.23E-10 4.43E-8 0.00E+0 3.18E-8 0.00E+0 0.00E+0 0.00E+0
10
SQP [-] ND ND ND ND ND ND ND ND ND ND ND ND ND ND
PM = Potential incidence of disease due to PM emissions; IR = Potential Human exposure efficiency relative to U235; ETP-fw = Potential
Caption comparative Toxic Unit for ecosystems; HTP-c = Potential comparative Toxic Unit for humans (cancerogenic); HTP-nc = Potential
comparative Toxic Unit for humans (not cancerogenic); SQP = Potential soil quality index
The SQP indicator is not given due to considerable uncertainties in the calculation.
The result figures given in module B2 refer to a period of 1 year because a reference service life is not declared.
They have to be multiplied by the assumed service life (in years) of the floor covering in the building under
consideration.
Disclaimer 1 – for the indicator “Potential Human exposure efficiency relative to U235”.
This impact category deals mainly with the eventual impact of low dose ionizing radiation on human health of the
nuclear fuel cycle. It does not consider effects due to possible nuclear accidents, occupational exposure or
radioactive waste disposal in underground facilities. Potential ionizing radiation from the soil, radon and from
some construction materials is also not measured by this indicator.
Disclaimer 2 – for the indicators “abiotic depletion potential for non-fossil resources”, “abiotic depletion potential
for fossil resources”, “water (user) deprivation potential, deprivation-weighted water consumption”, “potential
comparative toxic unit for ecosystems”, “potential comparative toxic unit for humans – cancerogenic”, “Potential
comparative toxic unit for humans - not cancerogenic”, “potential soil quality index”.
The results of this environmental impact indicator shall be used with care as the uncertainties on these results are
high as there is limited experience with the indicator.
References
EN 13501-1
DIN EN 13501-1:2019-05: Fire classification of ISO 14025
construction products and building elements - Part 1: DIN EN /ISO 14025:2011-10/, Environmental labels
Classification using data from reaction to fire tests and declarations — Type III environmental
declarations — Principles and procedures
EN 14041
DIN EN 14041: 2018-05: Resilient, textile and laminate ISO 14040
floor coverings - Essential characteristics DIN EN ISO 14040:2006+A1:2020 Environmental
management - Life cycle assessment - Principles and
EN 15804 framework
DIN EN 15804:2012+A2:2019+AC:2021, Sustainability
of construction works — Environmental Product
Declarations — Core rules for the product category of ISO 14044
construction products DIN EN ISO 14044:2006+A1:2018+A2:2020
Environmental management - Life cycle assessment -
EN 16810 Requirements and guidelines
DIN EN 16810: 2017-08: Resilient, textile and laminate
floor coverings – Environmental product declarations – ISO 10582
Product category rules DIN EN ISO 10582:2018-12 Elastische Bodenbeläge -
Heterogene Poly(vinylchlorid)-Bodenbeläge -
ISO 10874 Spezifikationen
DIN EN ISO 10874: 2012+A1:2021-04: Resilient,
textile and laminate floor coverings - Classification
7 Environmental Product Declaration Milliken – Luxury Vinyl Tiles (LVT) FlexForm™/FlexForm™ Sound
ISO 15686 26.07.2022, European Chemicals Agency (ECHA),
ISO 15686: Buildings and constructed assets - Helsinki, Finland
Service life planning
ISO 15686-1: 2011-05: Part 1: General principles and ecoinvent
framework ecoinvent, Zurich, Switzerland, database version 3.7,
ISO 15686-2: 2012-05: Part 2: Service life prediction published September 2020
procedures
ISO 15686-7: 2017-04: Part 7: Performance GaBi database
evaluation for feedback of service life data GaBi Software-System and Database for Life Cycle
from practice Engineering, thinkstep AG, Leinfelden-Echterdingen,
ISO 15686-8: 2008-06: Part 8: Reference service life 2022-1
and service-life estimation
PCR Part A
Regulation (EU) No. 305/2011 Product Category Rules for Building-Related Products
Regulation No. 305/2011 Construction Products and Services Part A: Calculation Rules for the Life
Regulation (CPR) of the European Council and of the Cycle Assessment and Requirements on the Project
European Parliament, April 2011 Report according to EN 15804+A2:2019, V1.2, Berlin:
Institut Bauen und Umwelt e.V. (IBU), November 2021
General Instructions for the IBU-EPD Program
General Instructions for the EPD-Program of the PCR Part B
Institut Bauen und Umwelt e.V., The Preparation of Product Category Rules for Building-Related Products
Environmental Product Declarations - EPDs, version and Services
2.0, Institut Bauen und Umwelt e.V., Berlin, January Part B: Requirements on the EPD for floor coverings,
2021, www.ibu-epd.de V1.2, Berlin: Institut Bauen und Umwelt e.V. (IBU), July
2022
BBSR
Bundesinstitut für Bau-, Stadt- und Raumforschung REACH
(BBSR) im Bundesamt für Bauwesen und Regulation (EC) No 1907/2006 of the European
Raumordnung (BBR), Bonn Parliament and of the Council of 18 December 2006
concerning the Registration, Evaluation, Authorisation
BNB, Nutzungsdauer von Bauteilen and Restriction of Chemicals (REACH), June 2017
Bewertungssystem Nachhaltiges Bauen (BNB),
Nutzungsdauer von Bauteilen, Bundesministerium des
Inneren, für Bau und Heimat, 24.02.2017
ECHA candidate list
Candidate List of substances of very high concern
(SVHCs) for authorisation, 08.07.2021, last update
8 Environmental Product Declaration Milliken – Luxury Vinyl Tiles (LVT) FlexForm™/FlexForm™ Sound
Publisher
Institut Bauen und Umwelt e.V. Tel +49 (0)30 3087748- 0
Hegelplatz 1 Fax +49 (0)30 3087748- 29
10117 Berlin Mail info@ibu-epd.com
Germany Web www.ibu-epd.com
Programme holder
Institut Bauen und Umwelt e.V. Tel +49 (0)30 - 3087748- 0
Hegelplatz 1 Fax +49 (0)30 – 3087748 - 29
10117 Berlin Mail info@ibu-epd.com
Germany Web www.ibu-epd.com
Author of the Life Cycle
Assessment Tel +49 (0)241 96843 410
Gemeinschaft umweltfreundlicher Fax +49 (0)241 96843 400
Teppichboden (GUT) e.V. Mail mail@gut-ev.de
Schönebergstraße 2 Web www.gut-ev.org
52068 Aachen
Germany
Owner of the Declaration
Milliken Industrials Ltd. Tel +44 (0) 1942 612777
Beech Hill Plant Fax .
Gidlow Lane Mail carpetenquiries@milliken.com
United Kingdom Web www.millikencarpet.com
