ENVIRONMENTAL PRODUCT DECLARATION
as per ISO 14025 and EN 15804+A2
Owner of the Declaration dormakaba International Holding GmbH
Publisher Institut Bauen und Umwelt e.V. (IBU)
Programme holder Institut Bauen und Umwelt e.V. (IBU)
Declaration number EPD-DOR-20220224-CBA1-EN
Issue date 29.11.2022
Valid to 28.11.2027
ESA 500 Automatic Sliding Door
Dormakaba
www.ibu-epd.com | https://epd-online.com
General Information
Dormakaba ESA 500 Automatic Sliding Door
Programme holder Owner of the declaration
IBU – Institut Bauen und Umwelt e.V. dormakaba International Holding GmbH
Hegelplatz 1 DORMA Platz 1
10117 Berlin 58256 Ennepetal
Germany Germany
Declaration number Declared product / declared unit
EPD-DOR-20220224-CBA1-EN 1 piece of the product: Automatic sliding door ESA 500 consisting of the
following items:
- header
- drive
- panels and jambs
- packaging material
This declaration is based on the product category rules: Scope:
Automatic doors, automatic gates, and revolving door systems, This EPD refers to a specific automatic sliding door ESA 500 produced by
01.08.2021 dormakaba USA Inc. The production site is located in Reamstown, PA
(PCR checked and approved by the SVR) USA.
The year of data collection is 2022.
Issue date The owner of the declaration shall be liable for the underlying information
and evidence; the IBU shall not be liable with respect to manufacturer
29.11.2022
information, life cycle assessment data and evidences.
The EPD was created according to the specifications of EN 15804+A2. In
Valid to
the following, the standard will be simplified as EN 15804.
28.11.2027
Verification
The standard EN 15804 serves as the core PCR
Independent verification of the declaration and data according to ISO
14025:2011
internally X externally
Dipl.-Ing. Hans Peters
(Chairman of Institut Bauen und Umwelt e.V.)
Florian Pronold Dr.-Ing. Wolfram Trinius,
(Managing Director Institut Bauen und Umwelt e.V.) (Independent verifier)
1 Environmental Product Declaration - Dormakaba - ESA 500 Automatic Sliding Door
Product
Product description/Product definition Delivery status:
The ESA 500 All Glass Automatic Sliding Door is perfect for The delivery status of an average ESA 500 Automatic Sliding
creating a glass look for interior applications. The ESA 500 Door includes header, drive, panels, jambs and packaging
sliding door is a superior choice for interior openings. The door materials:
solution is also recommended for exterior applications in
temperate climates. Suitable for larger openings with extended
width sidelites.
Features
• Breakout of sliding panels and sidelite
Base materials/Ancillary materials
• All Glass Look
The ESA 500 All Glass Automatic Sliding door comprises the
• Dual Vertical Weather Sweeps
following components:
• Factory Glazed 3/8' tempered glass
• Heavy-duty Delrin® and Brass Rollers
• Fully monitored overhead presence and activation
sensors
• Security interface
• Low maintenance
• High traffic volume
• Adjustable astragal
Optional Features
• Battery backup for keeping the door operational during
power loss
• Various thresholds to fit any site condition
• Transom
• Crash bars
The product contains partial articles which contain substances
• Glass stops up to 1"; sloped glass stops available
listed in the Candidate List of REACH
For placing especially on the market following standards are
Regulation 1907/2006/EC (date: 10.06.2022)
applicable:
exceeding 0.1 percentage by mass: no
• ICC/IBC International Building Code
• ANSI/BHMA A 156.10 American National Standard for Reference service life
Power Operated Doors Pedestrian Doors The life cycle of the ESA 500 door system is about 10 years,
• UL 325 Listed depending on the application and frequency of use. Regular
• NFPA 70 National Electrical Code maintenance is advised to ensure a life expectancy of 10 years.
• NFPA 101 Life Safety Code For repairs or renewals, suitable spare parts are available. The
• CUL Approved for use in Canada drive is tested to 1,000,000 closing cycles according to EN
16005.
Application
Recommended for interior and exterior applications in
temperate climates. Suitable for larger openings with extended
width sidelites. Applicable for single and double leaf doors.
Technical Data
The technical specification of the ESA 500 is as follows:
Constructional data
Name Value Unit
Height 240 mm
Installation depth 152 mm
Opening speed maximum 50 cm/s
Closing speed maximum 40 cm/s
Hold open time maximum 60 s
Supply voltage, frequency maximum 60 Hz
Power supply maximum 60 Hz
Internal power available 27 VDC/2A
Fuse 6.6 A
Power consumption maximum 250 W
2 Environmental Product Declaration - Dormakaba - ESA 500 Automatic Sliding Door
LCA: Calculation rules
Declared Unit Use stage - Module B6
The declared unit is 1 piece of the product: ESA 500 Automatic The use stage related to the operation of the building includes:
Sliding Door — B6, operational energy use
Declared unit
End-of-life stage– Modules C1-C4 and D
Name Value Unit
The end-of-life stage includes:
Declared unit 1 pce.
— C1, de-construction, demolition:
Mass (total system) 133,59 kg — C2, transport to waste processing;
— C3, waste processing for reuse, recovery and/or recycling;
System boundary — C4, disposal; including provision and all transport, provision
The type of EPD is: cradle-to-gate with options, modules C1– of all materials, products and related energy and water use.
C4, and module D (A1–A3 + C + D and additional modules: A4
+ A5 + B6) Module D (Benefits and loads beyond the system boundary)
includes:
Production - Module A1-A3 — D, recycling potentials, expressed as net impacts and
The product stage includes: benefits.
— A1, raw material extraction, processing and mechanical
Geographic Representativeness
treatments, processing of secondary material input (e.g.
Land or region, in which the declared product system is
recycling processes), — A2, transport to the manufacturer,
manufactured, used or handled at the end of the product´s
— A3, manufacturing and assembly including provision of all
lifespan: Global
materials, products and energy, as well as waste processing up
to the end-of-waste state.
Comparability
Construction stage - Modules A4-A5
Basically, a comparison or an evaluation of EPD data is only
The construction process stage includes:
possible if all the data sets to be compared were created
— A4, transport to the building site;
according to EN 15804 and the building context, respectively
— A5, installation into the building;
the product-specific characteristics of performance, are taken
including provision of all materials, products and energy, as well
into account. Background database: GaBi, SP40.
as waste processing up to the end-of waste state or disposal of
final residues during the construction process stage.
LCA: Scenarios and additional technical information
Reference service life
Characteristic product properties of biogenic carbon
Name Value Unit
Information on describing the Biogenic Carbon Content at
Life Span according to the manufacturer 10 a
factory gate
Name ValueUnit
kg
Biogenic carbon content in product 7.07
C Operational energy use (B6)
Biogenic carbon content in accompanying kg The use stage is declared for 10 years
0.74
packaging C Name Value Unit
Note: 1 kg of biogenic carbon is equivalent to 44/12 kg of CO . Electricity consumption for 1 year 189.29 kWh
2
Days per year in use 365 days
On mode per day 1.8 h
The following technical scenario information is required for the Idle mode per day 22.2 h
declared modules
On mode power 14,31 W
Transport from the gate to the site (A4)
Idle mode power 22.2 W
Name Value Unit
End of life (C1-C4)
Litres of fuel (per 1 kg) 0.00276 l/100km
Capacity utilisation (including empty runs) 55 % Name Value Unit
Transport distance via medium truck 100 km Collected separately waste type waste type 130.59 kg
Recycling 123 kg
The main distribution region is the american market. Transport
Energy recovery 4.14 kg
distance is declared for a distance of 100km by truck in order to
allow scaling to a specific point of installation. Landfilling 3.45 kg
Transport to waste management 50 km
Installation into the building (A5) The product is disassembled in a recycling process.
Name Value Unit Material recycling is then assumed for the metals, electronics
Waste packaging (paper and plastic) 3 kg and electromechanics. The plastic components are assumed to
be incinerated with energy recovery. Minor proportions of
residues arising from the recycling process are landfilled.
Region for the End of Life is: Global.
3 Environmental Product Declaration - Dormakaba - ESA 500 Automatic Sliding Door
Reuse, recovery and/or recycling potentials (D), relevant
scenario information
The collection rate is 100 %.
4 Environmental Product Declaration - Dormakaba - ESA 500 Automatic Sliding Door
LCA: Results
DESCRIPTION OF THE SYSTEM BOUNDARY (X = INCLUDED IN LCA; MND = MODULE OR INDICATOR NOT DECLARED; MNR
= MODULE NOT RELEVANT)
Benefits and
Construction loads beyond
Product stage Use stage End of life stage
process stage the system
boundaries
la ire ta m w a Ry lp p u s tro p s n a rT g n iru tc a fu n a M e h t m o rf tro p s n a rTe tis e h t o t e ta g y lb m e s s A e s U e c n a n e tn ia M ria p e R tn e m e c a lp e R tn e m h s ib ru fe R y g re n e la n o ita re p Oe s u re ta w la n o ita re p Oe s u n o itc u rts n o c -e Dn o itilo m e d tro p s n a rT g n is s e c o rp e ts a W la s o p s iD -e s u e R-y re v o c e R-g n ilc y c e Rla itn e to p
A1 A2 A3 A4 A5 B1 B2 B3 B4 B5 B6 B7 C1 C2 C3 C4 D
X X X X X MND X MNR MNR MNR X MND X X X X X
RESULTS OF THE LCA - ENVIRONMENTAL IMPACT according to EN 15804+A2: 1 piece ESA 500 Automatic Sliding Door
Parameter Unit A1-A3 A4 A5 B2 B6 C1 C2 C3 C4 D
GWP-total kg CO 2 eq 9.4E+02 1.17E+00 5.38E+00 0 1.06E+03 0 5.66E-01 4.58E+01 5.5E-02 -5.96E+02
GWP-fossil kg CO 2 eq 9.72E+02 1.12E+00 2.61E+00 0 1.06E+03 0 5.41E-01 1.1E+01 5.5E-02 -5.94E+02
GWP-
biogenic kg CO 2 eq -3.26E+01 5.2E-02 2.77E+00 0 2.3E-01 0 2.5E-02 3.48E+01 1.88E-04 -1.91E+00
GWP-luluc kg CO 2 eq 7E-01 2.66E-05 1.9E-04 0 3.21E-01 0 1.29E-05 9.28E-04 1.58E-04 -9.6E-02
ODP kg CFC11 eq 8.99E-09 1.18E-16 1.79E-15 0 3.74E-12 0 5.72E-17 9.53E-15 2.04E-16 -4.76E-09
AP mol H+ eq 4.5E+00 1E-03 1E-03 0 1.72E+00 0 5.42E-04 7E-03 3.95E-04 -2.24E+00
EP-
kg P eq 1.07E-03 2.39E-07 3.04E-07 0 5.81E-04 0 1.16E-07 1.47E-06 9.44E-08 -3.04E-04
freshwater
EP-marine kg N eq 6.23E-01 3.56E-04 3.89E-04 0 3.68E-01 0 1.72E-04 2E-03 1.02E-04 -2.93E-01
EP-terrestrial mol N eq 6.77E+00 4E-03 6E-03 0 3.95E+00 0 2E-03 3.2E-02 1E-03 -3.19E+00
kg NMVOC
POCP 1.93E+00 1E-03 1E-03 0 1.05E+00 0 4.88E-04 6E-03 3.08E-04 -9.24E-01
eq
ADPE kg Sb eq 4.22E-03 3.35E-08 2.57E-08 0 2.11E-04 0 1.62E-08 1.4E-07 4.94E-09 -5.62E-04
ADPF MJ 1.28E+04 1.58E+01 2.07E+00 0 1.72E+04 0 7.68E+00 1.23E+01 7.21E-01 -8.56E+03
m3 world eq
WDP 1.42E+02 2E-03 6.12E-01 0 2.06E+02 0 1E-03 4.7E+00 6E-03 -2.68E+01
deprived
GWP = Global warming potential; ODP = Depletion potential of the stratospheric ozone layer; AP = Acidification potential of land and water; EP =
Eutrophication potential; POCP = Formation potential of tropospheric ozone photochemical oxidants; ADPE = Abiotic depletion potential for non-fossil
resources; ADPF = Abiotic depletion potential for fossil resources; WDP = Water (user) deprivation potential)
RESULTS OF THE LCA - INDICATORS TO DESCRIBE RESOURCE USE according to EN 15804+A2: 1 piece ESA 500 Automatic
Sliding Door
Parameter Unit A1-A3 A4 A5 B2 B6 C1 C2 C3 C4 D
PERE MJ 5.4E+03 5E-02 2.45E+01 0 2.72E+03 0 2.4E-02 2.46E+02 9.5E-02 -4.09E+03
PERM MJ 2.67E+02 0 -2.4E+01 0 0 0 0 -2.43E+02 0 0
PERT MJ 5.67E+03 5E-02 4.69E-01 0 2.72E+03 0 2.4E-02 2.66E+00 9.5E-02 -4.09E+03
PENRE MJ 1.26E+04 1.59E+01 4.51E+01 0 1.72E+04 0 7.69E+00 1.26E+02 7.22E-01 -8.57E+03
PENRM MJ 1.57E+02 0 -4.3E+01 0 0 0 0 -1.14E+02 0 0
PENRT MJ 1.28E+04 1.59E+01 2.07E+00 0 1.72E+04 0 7.69E+00 1.23E+01 7.22E-01 -8.57E+03
SM kg 2.66E+00 0 0 0 0 0 0 0 0 0
RSF MJ 0 0 0 0 0 0 0 0 0 0
NRSF MJ 0 0 0 0 0 0 0 0 0 0
FW m3 1.27E+01 8.96E-05 1.4E-02 0 6.3E+00 0 4.34E-05 1.11E-01 1.82E-04 -7.08E+00
PERE = Use of renewable primary energy excluding renewable primary energy resources used as raw materials; PERM = Use of renewable primary
energy resources used as raw materials; PERT = Total use of renewable primary energy resources; PENRE = Use of non-renewable primary energy
excluding non-renewable primary energy resources used as raw materials; PENRM = Use of non-renewable primary energy resources used as raw
materials; PENRT = Total use of non-renewable primary energy resources; SM = Use of secondary material; RSF = Use of renewable secondary fuels;
NRSF = Use of non-renewable secondary fuels; FW = Use of net fresh water
RESULTS OF THE LCA – WASTE CATEGORIES AND OUTPUT FLOWS according to EN 15804+A2:
1 piece ESA 500 Automatic Sliding Door
Parameter Unit A1-A3 A4 A5 B2 B6 C1 C2 C3 C4 D
HWD kg 2.26E-05 1.54E-09 5.81E-09 0 6.63E-06 0 7.46E-10 2.38E-08 1.1E-08 -1.07E-05
NHWD kg 2.44E+02 2E-03 3.53E-01 0 5.35E+00 0 7.86E-04 1.34E+00 3.63E+00 -1.58E+02
RWD kg 7.48E-01 1.7E-05 9.08E-05 0 1.53E+00 0 8.25E-06 6.07E-04 8.21E-06 -9.72E-01
CRU kg 0 0 0 0 0 0 0 0 0 0
MFR kg 0 0 0 0 0 0 0 1.03E+02 0 0
MER kg 0 0 0 0 0 0 0 0 0 0
EEE MJ 0 0 9E+00 0 0 0 0 0 0 0
5 Environmental Product Declaration - Dormakaba - ESA 500 Automatic Sliding Door
EET MJ 0 0 1.86E+01 0 0 0 0 0 0 0
HWD = Hazardous waste disposed; NHWD = Non-hazardous waste disposed; RWD = Radioactive waste disposed; CRU = Components for re-use;
MFR = Materials for recycling; MER = Materials for energy recovery; EEE = Exported electrical energy; EET = Exported thermal energy
RESULTS OF THE LCA – additional impact categories according to EN 15804+A2-optional:
1 piece ESA 500 Automatic Sliding Door
Parameter Unit A1-A3 A4 A5 B2 B6 C1 C2 C3 C4 D
Disease
PM 4.68E-05 5.88E-09 1.02E-08 0 1.54E-05 0 2.85E-09 4.91E-08 4.88E-09 -3.62E-05
incidence
IR kBq U235 eq 1.47E+02 2E-03 1.1E-02 0 1.27E+02 0 1E-03 8.4E-02 8.45E-04 -1.96E+02
ETP-fw CTUe 4.62E+03 1.12E+01 8.67E-01 0 5.13E+03 0 5.44E+00 5.08E+00 4.12E-01 -3.22E+03
HTP-c CTUh 5.76E-07 2.11E-10 6.08E-11 0 1.1E-07 0 1.02E-10 3.77E-10 6.11E-11 -1.55E-07
HTP-nc CTUh 1.22E-05 9.03E-09 4.85E-09 0 4.17E-06 0 4.38E-09 2.36E-08 6.73E-09 -4.3E-06
SQP SQP 5.06E+03 4.1E-02 5.9E-01 0 1.57E+03 0 2E-02 3.53E+00 1.5E-01 -2.7E+02
PM = Potential incidence of disease due to PM emissions; IR = Potential Human exposure efficiency relative to U235; ETP-fw = Potential comparative
Toxic Unit for ecosystems; HTP-c = Potential comparative Toxic Unit for humans (cancerogenic); HTP-nc = Potential comparative Toxic Unit for humans
(not cancerogenic); SQP = Potential soil quality index
Disclaimer 1 – for the indicator IRP
This impact category deals mainly with the eventual impact of low dose ionizing radiation on human health of the nuclear fuel cycle. It
does not consider effects due to possible nuclear accidents, occupational exposure nor radioactive waste disposal in underground
facilities. Potential ionizing radiation from the soil, from radon and from some construction materials is also not measured by this
indicator.
Disclaimer 2 – for the indicators ADPE, ADPF, WDP, ETP-fw, HTP-c, HTP-nc, SQP
The results of this environmental impact indicator shall be used with care as the uncertainties on these results are high or as there is
limited experience with the indicator.
References
Standards EN 16005
DIN EN 16005: 2013-01, Power operated pedestrian doorsets -
A156.10 Safety in use - Requirements and test methods.
ANSI A156-2017 Power Operated Pedestrian Doors.
ICC/IBC
DIN 18650 The International Building Code (IBC) is a model building code
DIN 18650:2010, Powered pedestrian doors - Product developed by the International Code Council (ICC).
requirements and test methods.
NFPA 70
DIN EN 60335 National Electrical Code 70.
DIN EN 60335-1, -2-103:2020-08, Household and similar
electrical appliances - Safety - Part 1: General requirements. NFPA 101
Life Safety Code.
DIN EN 61000
DIN EN 61000-1-2:2017-07, Electromagnetic compatibility Further References
(EMC) - Part 1-2: General - Methodology for the achievement of
functional safety of electrical and electronic systems including 2011/65/EU ROHS3 Directive
equipment with regard to electromagnetic phenomena. Directive 2011/65/EU of the European Parliament and of the
Council of 8 June 2011 on the restriction of the use of certain
DIN EN 61508 hazardous substances in electrical and electronic equipment.
DIN EN 61508-2:2011-02, Functional safety of
electrical/electronic/programmable electronic safety-related IBU 2021
systems - Part 2: Requirements for General Instructions for the EPD programme of Institut Bauen
electrical/electronic/programmable electronic safety-related und Umwelt e.V.
systems. Version 2.0, Berlin: Institut Bauen und Umwelt e.V., 2021.
www.ibu-epd.com.
DIN EN ISO 13849
DIN EN ISO 13849-1:2021-08, Safety of machinery - Safety- GaBi ts software
related parts of control systems - Part 1: General principles for Sphera Solutions GmbH Gabi Software System and Database
design. for Life Cycle Engineering 1992-2020 Version 10.0.0.71
University of Stuttgart Leinfelden-Echterdingen.
DIN EN ISO 14025
DIN EN ISO 14025:2011-10, Environmental labels and GaBi ts documentation
declarations - Type III environmental declarations - Principles GaBi life cycle inventory data documentation
and procedures. (https://www.gabisoftware.
com/support/gabi/gabidatabase- 2020-lci-documentation/).
EN 15804
EN 15804+A2: 2019+AC:2021, Sustainability of construction LCA-tool dormakaba
works - Environmental Product Declarations - Core rules for the LCA tool, version ENS Door LCA tool No.: IBU-DOR-202107-
product category of construction products. LT1-EN Developed by Sphera Solutions GmbH.
6 Environmental Product Declaration - Dormakaba - ESA 500 Automatic Sliding Door
PCR Part A PCR Part B
PCR – Part A: Calculation Rules for the Life Cycle Assessment PCR – Part B: Requirements on the EPD for Building Hardware
and Requirements on the Project Re-port according to EN product, version 1.2, Institut Bauen und Umwelt e.V., www.ibu-
15804+A2:2019, Version 1.0, Institut Bauen und Umwelt e.V., epd.com, 2020.
www.ibu-epd.com.
7 Environmental Product Declaration - Dormakaba - ESA 500 Automatic Sliding Door
Publisher
Institut Bauen und Umwelt e.V. +49 (0)30 3087748- 0
Hegelplatz 1 info@ibu-epd.com
10117 Berlin www.ibu-epd.com
Germany
Programme holder
Institut Bauen und Umwelt e.V. +49 (0)30 3087748- 0
Hegelplatz 1 info@ibu-epd.com
10117 Berlin www.ibu-epd.com
Germany
Author of the Life Cycle Assessment
Sphera Solutions GmbH +49 711 341817-0
Hauptstraße 111- 113 info@sphera.com
70771 Leinfelden-Echterdingen www.sphera.com
Germany
Owner of the Declaration
dormakaba International Holding GmbH +49 2333 793-0
DORMA Platz 1 info.de@dormakaba.com
58256 Ennepetal www.dormakaba.com
Germany
8 Environmental Product Declaration - Dormakaba - ESA 500 Automatic Sliding Door
