ENVIRONMENTAL PRODUCT DECLARATION
as per ISO 14025 and EN 15804+A2
Owner of the Declaration Ideal Standard International NV
Publisher Institut Bauen und Umwelt e.V. (IBU)
Programme holder Institut Bauen und Umwelt e.V. (IBU)
Declaration number EPD-IDE-20230127-IBB1-EN
Issue date 20.12.2023
Valid to 19.12.2028
Ceramic cistern
Ideal Standard International
www.ibu-epd.com | https://epd-online.com
1. General Information
Ideal Standard International Ceramic cistern
Programme holder Owner of the declaration
IBU – Institut Bauen und Umwelt e.V. Ideal Standard International NV
Hegelplatz 1 Da Vincilaan 2
10117 Berlin 1935 Zaventem
Germany Belgium
Declaration number Declared product / declared unit
EPD-IDE-20230127-IBB1-EN One piece of cistern, including one tank trim.
This declaration is based on the product category rules: Scope:
Sanitary ceramics, 01.08.2021
(PCR checked and approved by the SVR) The EPD contains the result for 1 piece of cistern produced by IS.
As the cistern can be produced in 3 different ceramic plants, respectively:
Sevlievo (Bulgaria), Armitage (United Kingdom) and Teplice (Czech
Issue date Republic), the LCA results are based on the weighted average data.
In the LCA report, a variability study between the average and the three
20.12.2023
specific plants has been included.
Valid to
Note that the results have been separated for the ceramic part and the
19.12.2028 tank trim, so the user can easily calculate the results for a cistern with a
different weight. The formula is described further in this document.
Foreground data has been provided directly by Ideal Standard and
background LCA data is based on Ecoinvent 3.8 and Industry 2.0 data.
The owner of the declaration shall be liable for the underlying information
and evidence; the IBU shall not be liable with respect to manufacturer
information, life cycle assessment data and evidences.
The EPD was created according to the specifications of EN 15804+A2. In
the following, the standard will be simplified as EN 15804.
Verification
Dipl.-Ing. Hans Peters The standard EN 15804 serves as the core PCR
(Chairman of Institut Bauen und Umwelt e.V.)
Independent verification of the declaration and data according to ISO
14025:2011
internally X externally
Florian Pronold Vito D'Incognito,
(Managing Director Institut Bauen und Umwelt e.V.) (Independent verifier)
1 Environmental Product Declaration - Ideal Standard International - Ceramic cistern
2. Product
2.1 Product description/Product definition 2.5 Base materials/Ancillary materials
The product under study is a standard white porcelain cistern, The main components of the cistern product is: ceramic and the
including the tank trim (i.e. inlet and outlet valve of the flushing tank trim.
mechanism). The EPD contains the result for 1 piece of cistern This detailed composition of ceramic is as the relevant:
produced by IS. 20-30% clay,
As the cistern can be produced in 3 different ceramic plants, 20-30% China clay
respectively: Sevlievo (Bulgaria), Armitage (United Kingdom) 20-30% Feldspar
and Teplice (Czech Republic), the LCA results are based on the 20-30% Silica
weighted average data. In the LCA report, a variability study <5% Glaze
between the average and the 3 specific plants has been
included. The composition of the tank trim :
· +/- 90% plastics (mainly ABS, but also POM, PE and PP)
The manufacturer can - within the framework of the European · +/- 10% steel/brass
Regulation N° 305/2011 (CPR) - present the Declaration of
Performance (DOP) of the product confirming that the product This product does not contain any substances listed in the
has a CE marking. candidate list (date: 26.10.2022) exceeding 0.1 percentage by
mass.
For the application and use the respective national provisions
apply. This product does not contain other CMR substances in
categories 1A or 1B which are not on the candidate list,
2.2 Application exceeding 0.1 percentage by mass,
The product is used in private and public bathrooms. The
product can be used in new construction and renovation work Biocide products were not added to this construction product
for hygienic and household use. and it has not been treated with biocide products as defined by
the (EU) Ordinance on Biocide Products No. 528/2012.
2.3 Technical Data
2.6 Manufacture
Constructional data 1. Slip preparation
Production of the ceramic mixture (slip) and unloading/storage
Name Value Unit
of raw materials in the area.
Minimum 1
Crazing test Internal test - 1hr in autoclave
cycle without -
with 5bar steam 2. Glaze preparation
crazing
Production of glaze with needed color.
Water absorption EN997 for WC pans
(toilets) and so by extension to the <0.5 % 3. Casting shop
Vitreous China products Casting of ceramic products in different moulds.
Minimum 1
Impact resistance Internal test – Ball
drop without - 4. Dryers
bearing dropped from fixed height
breaking The drying is process of taking off the humidity and the final
Resistance to temperature change EN result are dried products.
14688 for Wash Basins. 1000 hot (75 No visible
degC) / cold (15 degC) water cycles damage - 5. White inspection
without visible damage The first inspection of dried ceramic products. The main focus
is checking the quality
Resistance to chemicals and staining EN
and cleaning the surface of the products. At the end of the
14688 for Wash Basins therefore by
No remaining process the products are grouping in three different directions:
extension to other Ceramic Products.
chemical - A grade products, for repairing and scrap.
Specific chemicals in contact then cleaned
evident
with specific apparatus without permanent
marking
6. Spraying
Resistance to abrasion EN 14688 for
Covering the ceramic product with glaze
Wash Basins therefore by extension to No scratches
other Ceramic Products. Loaded diamond through outer -
7. Kilns
tool (scratch) / Loaded abrasive paper (glaze) layer
Firing of ceramic products
wheel (abrasion) for repeated cycles.
Load resistance 400 kg 8. Gloss inspection
Final inspection for visual control of all products for defects
2.4 Delivery status presence. Separating the products again in three groups: for
The products are packed: wooden pallet, PE plastic foil and packaging, for repairing by hand or grinding machines and
coverage carton, and are accompanied with an instruction and scrap (pitcher).
guarantee sheet.
The products can come in different shapes and dimensions. An 9. Packaging
overview of all different cisterns can be found on Ideal Different kind of activities for packaging of the products.
Standard's website and filter on 'Cisterns':
https://www.idealstandard.co.uk/products/catalog/toilets/cisterns *Moulds making
Development of new matrix for production of gypsum moulds
2 Environmental Product Declaration - Ideal Standard International - Ceramic cistern
for casting and repairing of damaged matrix.
2.11 Environment and health during use
*Mould shop Under normal conditions of use, the product do not cause any
Production of gypsum moulds for casting the ceramic products adverse health effects or release of volatile organic compounds
and polyurethane setters for supporting the casting process. (VOCs) into indoor air. No environmental impact on water, air or
soil is expected.
2.7 Environment and health during manufacturing
Environmental, occupational health, safety and quality 2.12 Reference service life
management at the Ideal Standard plants The reference service life is not included, as module B is not
are in accordance with the following standards: considered.
· ISO 14001 Description of the influences on the ageing of the product when
· ISO 9001 applied in accordance with the rules of technology.
· ISO 45001
2.8 Product processing/Installation 2.13 Extraordinary effects
It is considered that there is no assembly waste, based on the Fire
fact that the product is prefabricated and installed by hand. Fire
Not subjected to fire classification
2.9 Packaging
A wooden pallet, PE plastic bag and coverage carton are used
to pack and transport the product to the supplier/customer. The Water
product is also accompanied with an instruction sheet. No risks are expected to occur in terms of environmental and
human health.
Mechanical destruction
In case of mechanical destruction, no risks are expected to
occur in terms of environment and human health.
2.14 Re-use phase
It is possible to partially recycle ceramic products in the
production process. This is already applied for production
waste. The recycling of post-consumer waste depends on the
sorting and take-back of these waste streams at the demolition
site.
2.15 Disposal
According to the average European end-of-life scenario
described in Annex C of the Product Environmental Footprint
Pilots (PEFCR) 6.3 guidance (version March 2018), the
following disposal scenarios have been considered: 100% of
the ceramic is landfilled, 45% of the plastic parts are incinerated
and 55% of the plastic parts are landfilled.
2.16 Further information
Additional information on cisterns produced by Ideal Standard
2.10 Condition of use
can be found at:
The product will not change in material composition during use.
https://www.idealstandard.co.uk/products/catalog/toilets/cisterns
3. LCA: Calculation rules
Then, other cisterns can be calculated by weight interpolation
3.1 Declared Unit of the ceramic parts. The environmental impact of the cistern
will be presented separately for the ceramic parts and the tank
Declared unit cisterns that include a cistern with another weight. Therefore,
the following formula should be used:
Name Value Unit
Mass per piece 11.69 kg
Declared unit 1 Piece
Mass of the ceramic cistern 11 Kg
Mass of the tank trim 0.69 Kg
Mass reference 11.69 kg/pce EB = Environmental impact of the ceramic parts of a specific
cistern,
The weight of the cistern is based on a specific one, the most
ER = Environmental impact of the ceramic parts of the
sold by Ideal Standard in 2021 in BG52. The results for cisterns
reference cistern,
with another weight can be calculated using the Annex, in
WR = Weight of the ceramic parts of the reference product,
which the results for 1 kg ceramic and 1 piece Tank trim have
WB = Weight of the ceramic parts of a specific cistern,
been described separately.
3 Environmental Product Declaration - Ideal Standard International - Ceramic cistern
ensure a comfortable indoor climate for the personnel for
3.2 System boundary example is also neglected.
Cradle-to-gate with options, including module D.
3.5 Background data
3.3 Estimates and assumptions Ecoinvent 3.8 and Industry 2.0
The following processes are excluded because data was not
available: 3.6 Data quality
· Packaging of the following raw materials used to produce the Foreground data is specific to Ideal Standard and is collected
glaze of the ceramic products: barium carbonate, sodium for the reference year 2021. Background data is based on
carbonate, sodium silicate, aluminium hydroxide, Ecoinvent 3.8 which is released in September 2021, and
aluminium oxide, zinc oxide and stains Industry 2.0. The LCA background report includes details on the
weighted average data of the different factory plants,
· Transport packaging final product respectively Sevlievo (Bulgaria), Armitage (United Kingdom)
and Teplice (Czech Republic).
· Packaging and transport of ancillary materials used during the
production process 3.7 Period under review
The data collected by Ideal Standard is based on data from the
· Packaging and transport of ancillary materials used during production year 2021 for both the ceramics and the tank trim.
installation
3.8 Geographic Representativeness
No further approximations have been made to replace the Land or region, in which the declared product system is
missing data, as they were manufactured, used or handled at the end of the product´s
considered to be not relevant based on the first iterations of the lifespan: Global
results.
3.9 Allocation
3.4 Cut-off criteria
EN15804+A2 also describes the rules for joint co-production,
· Big bags used as packaging of some raw materials for the
where the processes cannot be divided. This is, however, not
ceramic production, as they are reused.
the case in this study. Allocation of secondary materials or
secondary fuels is also not applicable for this study.
· Only most relevant ancillary materials have been selected
based on consumption rate and
3.10 Comparability
importance in the production process.
Basically, a comparison or an evaluation of EPD data is only
possible if all the data sets to be compared were created
· Environmental impacts caused by the personnel of the
according to EN 15804 and the building context, respectively
production plants are not included in the LCA, e.g. waste from
the product-specific characteristics of performance, are taken
the cafeteria and sanitary installations, accidental pollution
into account. Ecoinvent 3.8 and Industry 2.0.
caused by human mistakes, or environmental effects caused by
commuter traffic. Heating or cooling of the plants in order to
4. LCA: Scenarios and additional technical information
Transport to the building site (A4)
Characteristic product properties of biogenic carbon
The product does not contain biogenic carbon, but its Name Value Unit
accompanying packaging (of ceramic parts and tank trim) Litres of fuel 25.4 l/100km
contains 9.49E-01kg C per product in the form of paper, Transport distance 2000 Km
cardboard and wooden pallets.
Capacity utilisation (including Default value
%
Information on describing the biogenic carbon content at empty runs) Ecoinvent
factory gate Gross density of products
Not calculated kg/m3
Name ValueUnit transported
kg
Biogenic carbon content in product - Installation into the building (A5)
C
Name Value Unit
Biogenic carbon content in accompanying kg
packaging 0.949 C Packaging waste (paper and cardboard) PEF
EOL scenario Europe for coverage carton 8.19E-
Note: 1 kg of biogenic carbon is equivalent to 44/12 kg of CO2. Kg
packaging: 11% incineration; 75% recycling; 14% 01
landfill
Packaging waste (PE) PEF EOL scenario Europe
3.99E-
for PE packaging: 32% incineration; 29% Kg
01
recycling; 39% landfill
Packaging waste (wooden pallet) PEF EOL
1.31E
scenario Europe for wooden pallets: 32% Kg
+00
incineration; 30% recycling; 38% landfill
End of life (C1-C4)
According to the average European end-of-life scenario
described in Annex C of the Product Environmental Footprint
4 Environmental Product Declaration - Ideal Standard International - Ceramic cistern
Pilots (PEFCR) 6.3 guidance (version March 2018), the
Reuse, recovery and/or recycling potentials (D), relevant
following disposal scenarios have been considered: 100% of
scenario information
the ceramic parts are landfilled, 45% of the plastic parts are
Module D contains the benefits and loads of recycling the
incinerated, 55% of the plastic parts are landfilled, 95% of the
smaller metal parts and the benefits of energy recovery during
smaller metal parts are recycled and 5% of the smaller metal
the incineration of the plastics.
parts are landfilled.
Name ValueUnit
Name Value Unit
Loads recycling of brass: Impact of the production
Collected as mixed construction waste 11,69 Kg
process of brass excluding the production of raw 0.051 Kg
Reuse 0 Kg
materials
Landfill of ceramics (from cistern) 11 Kg
Benefits recycling of brass: Avoided production of
0.051 Kg
Landfill of plastics (from tank trim) 0.347 Kg brass using 100% primary materials
Landfill of metals (from tank trim) 0.003 Kg Benefits energy recovery during incineration of
Incineration of plastics (from tank trim) 0.284 Kg plastics from tank trim: 20% avoided production of 1.75 MJ
Recycling of metals (from tank trim) 0.051 Kg Heat from natural gas
Benefits energy recovery during incineration of
plastics from tank trim: 10% avoided production of 0.88 MJ
European average grid mix
5 Environmental Product Declaration - Ideal Standard International - Ceramic cistern
5. LCA: Results
An annex is added to this EPD in which the environmental impact is presented separately for 1 kg ceramics and 1 piece of tank trim,
allowing the user to calculate the environmental impact of a cistern with another different weight.
DESCRIPTION OF THE SYSTEM BOUNDARY (X = INCLUDED IN LCA; MND = MODULE OR INDICATOR NOT DECLARED; MNR
= MODULE NOT RELEVANT)
Benefits and
Construction loads beyond
Product stage Use stage End of life stage
process stage the system
boundaries
la ire ta m w a Ry lp p u s tro p s n a rT g n iru tc a fu n a M e h t m o rf tro p s n a rTe tis e h t o t e ta g y lb m e s s A e s U e c n a n e tn ia M ria p e R tn e m e c a lp e R tn e m h s ib ru fe R y g re n e la n o ita re p Oe s u re ta w la n o ita re p Oe s u n o itc u rts n o c -e Dn o itilo m e d tro p s n a rT g n is s e c o rp e ts a W la s o p s iD -e s u e R-y re v o c e R-g n ilc y c e Rla itn e to p
A1 A2 A3 A4 A5 B1 B2 B3 B4 B5 B6 B7 C1 C2 C3 C4 D
X X X X X MND MND MNR MNR MNR MND MND X X X X X
RESULTS OF THE LCA - ENVIRONMENTAL IMPACT according to EN 15804+A2: 1 Piece Cistern including a tank trim
Parameter Unit A1 A2 A3 A4 A5 C1 C2 C3 C4 D
GWP-total kg CO 2 eq 2.63E+00 1.36E+00 1.41E+01 4.63E+00 3.75E+00 1.69E-03 1.06E-01 7.8E-05 7.79E-01 -2.02E+00
GWP-fossil kg CO 2 eq 2.61E+00 1.36E+00 1.72E+01 4.63E+00 4.8E-01 1.67E-03 1.06E-01 7.73E-05 7.79E-01 -4.89E-01
GWP-
biogenic kg CO 2 eq 8.47E-03 4.41E-04 -3.18E+00 1.66E-03 3.27E+00 9.29E-06 3.78E-05 4.19E-07 1.6E-04 -1.53E+00
GWP-luluc kg CO 2 eq 2.08E-03 6.59E-04 1.05E-02 1.85E-03 3.47E-05 3.96E-06 4.23E-05 1.79E-07 6.54E-05 -1.8E-03
ODP kg CFC11 eq 2.42E-07 3.03E-07 1.81E-06 1.07E-06 1.77E-08 8.43E-11 2.45E-08 4.01E-12 3.04E-08 -8.04E-08
AP mol H+ eq 1.3E-02 1.42E-02 5.28E-02 1.31E-02 4.64E-04 9.52E-06 3E-04 4.43E-07 7.96E-04 -3.24E-03
EP-
kg P eq 1.45E-04 8.45E-06 1.12E-03 3.3E-05 9.07E-07 1.79E-07 7.54E-07 8.11E-09 2.59E-06 -4.43E-05
freshwater
EP-marine kg N eq 1.97E-03 3.36E-03 9.36E-03 2.61E-03 1.79E-04 1.21E-06 5.97E-05 5.9E-08 3.26E-04 -6.17E-04
EP-terrestrial mol N eq 2.22E-02 3.73E-02 9.77E-02 2.91E-02 1.81E-03 1.4E-05 6.65E-04 6.78E-07 3.13E-03 -6.88E-03
kg NMVOC
POCP 7.13E-03 1.05E-02 2.83E-02 1.12E-02 5.43E-04 3.84E-06 2.56E-04 1.9E-07 8.76E-04 -1.8E-03
eq
ADPE kg Sb eq 3.78E-05 3.11E-06 1.58E-05 1.25E-05 2.12E-07 9.05E-09 2.86E-07 4.38E-10 2.42E-07 -1.66E-05
ADPF MJ 5.53E+01 1.98E+01 3.27E+02 7.02E+01 1.2E+00 3.55E-02 1.6E+00 1.62E-03 2.14E+00 -3.79E+00
m3 world eq
WDP 1.88E+00 5.43E-02 5.15E+00 2.14E-01 7.1E-03 4.15E-04 4.88E-03 1.9E-05 1.74E-02 -3.57E-01
deprived
GWP = Global warming potential; ODP = Depletion potential of the stratospheric ozone layer; AP = Acidification potential of land and water; EP =
Eutrophication potential; POCP = Formation potential of tropospheric ozone photochemical oxidants; ADPE = Abiotic depletion potential for non-fossil
resources; ADPF = Abiotic depletion potential for fossil resources; WDP = Water (user) deprivation potential)
RESULTS OF THE LCA - INDICATORS TO DESCRIBE RESOURCE USE according to EN 15804+A2: 1 Piece Cistern including a
tank trim
Parameter Unit A1 A2 A3 A4 A5 C1 C2 C3 C4 D
PERE MJ 3.97E+00 2.45E-01 1.75E+01 9.87E-01 7.34E+00 7.06E-03 2.25E-02 3.18E-04 1.18E-01 0
PERM MJ 3.04E-02 0 3.13E+01 0 -2.26E+01 0 0 0 0 1.53E+01
PERT MJ 4E+00 2.45E-01 4.88E+01 9.87E-01 -1.52E+01 7.06E-03 2.25E-02 3.18E-04 1.18E-01 1.53E+01
PENRE MJ 4.82E+01 1.98E+01 3.57E+02 7.06E+01 6.65E+00 4.22E-02 1.61E+00 1.92E-03 8.26E+00 0
PENRM MJ 1.35E+01 0 1.69E+01 0 -1.03E+01 0 0 0 -6.04E+00 4.93E+00
PENRT MJ 6.17E+01 1.98E+01 3.73E+02 7.06E+01 -3.68E+00 4.22E-02 1.61E+00 1.92E-03 2.22E+00 4.93E+00
SM kg 2.79E-01 0 0 0 0 0 0 0 0 8.99E-01
RSF MJ 0 0 0 0 0 0 0 0 0 0
NRSF MJ 0 0 0 0 0 0 0 0 0 0
FW m3 1.63E-01 1.27E-03 1.03E-01 5.16E-03 6.26E-04 2.68E-05 1.18E-04 1.21E-06 2.46E-03 -1.31E-02
PERE = Use of renewable primary energy excluding renewable primary energy resources used as raw materials; PERM = Use of renewable primary
energy resources used as raw materials; PERT = Total use of renewable primary energy resources; PENRE = Use of non-renewable primary energy
excluding non-renewable primary energy resources used as raw materials; PENRM = Use of non-renewable primary energy resources used as raw
materials; PENRT = Total use of non-renewable primary energy resources; SM = Use of secondary material; RSF = Use of renewable secondary fuels;
NRSF = Use of non-renewable secondary fuels; FW = Use of net fresh water
RESULTS OF THE LCA – WASTE CATEGORIES AND OUTPUT FLOWS according to EN 15804+A2:
1 Piece Cistern including a tank trim
Parameter Unit A1 A2 A3 A4 A5 C1 C2 C3 C4 D
HWD kg 7.16E-05 4.42E-05 3.11E-04 1.83E-04 2.89E-06 2.7E-08 4.18E-06 1.33E-09 2.7E-06 -2.33E-05
NHWD kg 7.5E-01 8.14E-01 1.76E+00 3.68E+00 8.29E-01 1.3E-04 8.4E-02 6.3E-06 1.14E+01 -8.68E-02
RWD kg 1.43E-04 1.34E-04 9.91E-04 4.74E-04 7.79E-06 2.59E-07 1.08E-05 1.18E-08 1.42E-05 -5.16E-05
CRU kg 0 0 0 0 0 0 0 0 0 0
MFR kg 0 0 4.23E-03 0 1.12E+00 0 0 5.13E-02 0 -1.18E+00
6 Environmental Product Declaration - Ideal Standard International - Ceramic cistern
MER kg 0 0 0 0 0 0 0 0 0 0
EEE MJ 0 0 1.48E-03 0 1.22E+00 0 0 0 2.83E-01 -1.51E+00
EET MJ 0 0 2.95E-03 0 2.45E+00 0 0 0 5.65E-01 -3.02E+00
HWD = Hazardous waste disposed; NHWD = Non-hazardous waste disposed; RWD = Radioactive waste disposed; CRU = Components for re-use;
MFR = Materials for recycling; MER = Materials for energy recovery; EEE = Exported electrical energy; EET = Exported thermal energy
RESULTS OF THE LCA – additional impact categories according to EN 15804+A2-optional:
1 Piece Cistern including a tank trim
Parameter Unit A1 A2 A3 A4 A5 C1 C2 C3 C4 D
Disease
PM 9.36E-08 9.2E-08 3.73E-07 3.72E-07 8.13E-09 2.62E-11 8.49E-09 1.48E-12 1.33E-08 -4.76E-08
incidence
IR kBq U235 eq 2.85E-01 8.56E-02 1.21E+00 3.05E-01 5.34E-03 3.15E-04 6.96E-03 1.42E-05 1.08E-02 -5.66E-02
ETP-fw CTUe 6.4E+01 1.48E+01 7.67E+01 5.51E+01 1.29E+00 2.25E-02 1.26E+00 1.07E-03 3.09E+00 -1.44E+01
HTP-c CTUh 3.68E-09 5.97E-10 6.22E-09 1.77E-09 2.32E-10 6.9E-13 4.05E-11 5.4E-14 1.69E-10 -3.59E-10
HTP-nc CTUh 5.27E-08 1.39E-08 1.09E-07 5.57E-08 1.8E-09 2.2E-11 1.27E-09 1.06E-12 1.97E-09 -2.86E-08
SQP SQP 1.95E+01 1.13E+01 2.49E+02 4.89E+01 1.1E+00 6.43E-03 1.12E+00 1.06E-03 3.85E+00 -1.63E+02
PM = Potential incidence of disease due to PM emissions; IR = Potential Human exposure efficiency relative to U235; ETP-fw = Potential comparative
Toxic Unit for ecosystems; HTP-c = Potential comparative Toxic Unit for humans (cancerogenic); HTP-nc = Potential comparative Toxic Unit for humans
(not cancerogenic); SQP = Potential soil quality index
Disclaimer 1 – for the indicator 'Potential Human exposure efficiency relative to U235'. This impact category deals mainly with the
eventual impact of low-dose ionizing radiation on human health of the nuclear fuel cycle. It does not consider effects due to possible
nuclear accidents, occupational exposure or radioactive waste disposal in underground facilities. Potential ionizing radiation from the
soil, radon and from some construction materials is also not measured by this indicator.
Disclaimer 2 – for the indicators 'abiotic depletion potential for non-fossil resources', 'abiotic depletion potential for fossil resources',
'water (user) deprivation potential, deprivation-weighted water consumption', 'potential comparative toxic unit for ecosystems', 'potential
comparative toxic unit for humans – cancerogenic', 'Potential comparative toxic unit for humans - not cancerogenic', 'potential soil
quality index'. The results of this environmental impact indicator shall be used with care as the uncertainties on these results are high
as there is limited experience with the indicator.
An annex is added to this EPD in which the environmental impact is presented separately for 1 kg ceramics and 1 piece of tank trim,
allowing the user to calculate the environmental impact of a cistern with another different weight.
6. LCA: Interpretation
For the cistern, more than 90% of the impact is related to the
ceramic parts in the case of a
total ceramic weight of 11 kg. However, note that the
contribution of the tank trim will increase with decreasing For the tank trim, the raw materials or module A1 has the
weights of the ceramic parts. largest contribution on all impact categories. The second most
important module, is module A3 or the manufacturing process.
For the ceramic parts, the manufacturing or module A3 (and in Outside the system's boundaries, module D shows the benefits
particular the energy consumption) has the largest contribution from the energy recovery from incineration of the plastic
on all impact categories. Besides the manufacturing, also the components and to a lesser extend the recycling of the small
transport to the installation site has a significant contribution, steel components in the tank trim. In module D the use of
due to the weight of the product. The impact of the raw recycled content at the beginning of life has been taken into
materials is less significant. account in the calculations, as required by EN15804+A2.
7. Requisite evidence
8. References
Standards Institut Bauen und Umwelt e.V, Berlin (pub.): PCR Guidance-
Texts for Building-Related Products and Services From the
EN15804 range of Environmental Product Declarations of Institute
Construction and Environment e.V. (IBU) : Requirements on the
EN 15804:2012+A2:2019+AC:2021, Sustainability of EPD for Sanitary ceramics, version 4 (19/10/2023)
construction works — Environmental
Product Declarations — Core rules for the product category of ISO 9001
construction products. ISO 9001:2015: Quality management systems — Requirements
PCR Part A ISO 14001
Calculation rules for the Life Cycle Assessment and ISO 14001:2015: Environmental management systems —
Requirements on the Background Report, Institut Bauen und Requirements with guidance for use
Umwelt e.V., www.bauumwelt.com. Version 1.3
ISO 14025
PCR Part B EN ISO 14025:2011, Environmental labels and declarations —
7 Environmental Product Declaration - Ideal Standard International - Ceramic cistern
Type III environmental declarations — Principles and 21(9), pp.1218–1230.
procedures. .
ISO 14040 Industry 2.0
ISO 14040:2006: Environmental management – Life cycle Industry 2.0 (from PlasticsEurope, worldsteel and ERASM) LCA
assessment – Principles and framework. database as integrated in SimaPro 9.3.0.3.
ISO 14044 PEFCR
ISO 14044:2006: Environmental management – Life cycle European commission (2018). Product Environmental Footprint
assessment – Requirements and guidelines. Category Rules PEFCR Guidance, version 6.3.
ISO 45001
ISO 45001:2018: Occupational health and safety management IBU
systems Requirements with guidance for use IBU 2021. Institut Bauen und Umwelt e.V.: General Instructions
for the EPD programme of Institut Bauen und Umwelt e.V.,
Further references Version 2.0, Berlin: Institut Bauen und Umwelt e.V., 2021
www.ibu-epd.com
Pré Consultants REACH candidate list
(2021) SimaPro ECHA, REACH Candidate List of substances of very
9.3.0.3 [Computer Software]. Amersfoort, The Netherlands. highconcern for Au
Biocide Products No. 528/2012EU, REGULATION (EU) No
CPR 528/2012 OF THE EUROPEANPARLIAME
European Regulation N° 305/2011 (CPR)
Ecoinvent The literature referred to in the Environmental Product
Wernet, G., Bauer, C., Steubing, B., Reinhard, J., Moreno-Ruiz, Declaration must be listed in full.Standards already fully quoted
E., and Weidema, B., 2016. The ecoinvent database version 3 in the EPD do not need to be listed here again.
(part I): overview and methodology. The International Journal of The current version of PCR Part A and PCR Part B of the PCR
Life Cycle Assessment, [online] document on which they are based must be referenced.
8 Environmental Product Declaration - Ideal Standard International - Ceramic cistern
Publisher
Institut Bauen und Umwelt e.V. +49 (0)30 3087748- 0
Hegelplatz 1 info@ibu-epd.com
10117 Berlin www.ibu-epd.com
Germany
Programme holder
Institut Bauen und Umwelt e.V. +49 (0)30 3087748- 0
Hegelplatz 1 info@ibu-epd.com
10117 Berlin www.ibu-epd.com
Germany
Author of the Life Cycle Assessment
Ideal Standard International NV +32(0)28004800
Da Vincilaan 2 eboukari@idealstandard.com
1935 Zaventem www.idealstandard.com
Belgium
Owner of the Declaration
Ideal Standard International NV +32(0)28004800
Da Vincilaan 2 eboukari@idealstandard.com
1935 Zaventem www.idealstandard.com
Belgium
9 Environmental Product Declaration - Ideal Standard International - Ceramic cistern
