ENVIRONMENTAL PRODUCT DECLARATION
as per ISO 14025 and EN 15804+A2
Owner of the Declaration dormakaba International Holding GmbH
Publisher Institut Bauen und Umwelt e.V. (IBU)
Programme holder Institut Bauen und Umwelt e.V. (IBU)
Declaration number EPD-DOR-20220211-CBA1-EN
Issue date 29.11.2022
Valid to 28.11.2027
ESA 100-300 Automatic Sliding Door
Dormakaba
www.ibu-epd.com | https://epd-online.com
General Information
Dormakaba ESA 100-300 Automatic Sliding Door
Programme holder Owner of the declaration
IBU – Institut Bauen und Umwelt e.V. dormakaba International Holding GmbH
Hegelplatz 1 DORMA Platz 1
10117 Berlin 58256 Ennepetal
Germany Germany
Declaration number Declared product / declared unit
EPD-DOR-20220211-CBA1-EN 1 piece of the product: Automatic Sliding Door consisting of the following
items:
- header
- drive
-panels and jambs
- packaging material
This declaration is based on the product category rules: Scope:
Automatic doors, automatic gates, and revolving door systems, This EPD refers to a specific automatic sliding door (ESA 200) produced
01.08.2021 by dormakaba USA Inc. The production site is located in Reamstown, PA
(PCR checked and approved by the SVR) USA. The EPD is also representative for the ESA 100 and 300 sliding
doors.
The year of data collection is 2022.
Issue date The owner of the declaration shall be liable for the underlying information
and evidence; the IBU shall not be liable with respect to manufacturer
29.11.2022
information, life cycle assessment data and evidences.
The EPD was created according to the specifications of EN 15804+A2. In
Valid to
the following, the standard will be simplified as EN 15804.
28.11.2027
Verification
The standard EN 15804 serves as the core PCR
Independent verification of the declaration and data according to ISO
14025:2011
internally X externally
Dipl.-Ing. Hans Peters
(Chairman of Institut Bauen und Umwelt e.V.)
Florian Pronold Dr.-Ing. Wolfram Trinius,
(Managing Director Institut Bauen und Umwelt e.V.) (Independent verifier)
1 Environmental Product Declaration - Dormakaba - ESA 100-300 Automatic Sliding Door
Product
Product description/Product definition
ESA 200 Commercial Fixed Sidelite Door
Extruded aluminium stile and rail door; for interior or exterior
applications.
Recommended for large opening applications. Reduced air
Base materials/Ancillary materials
infiltration allows handling of windy conditions. Egress capacity
The ESA 200 automatic sliding door comprises the following
comparable to standard swing doors.
components, the same as ESA 100 and ESA 300:
Features
• Breakout of sliding panels only
• Narrow or medium stile
• Performance glass options
• Heavy-duty Delrin® and Brass Rollers
• Fully monitored overhead presence and activation
sensors
• Security interface
• Low maintenance
The product contains partial articles which contain substances
• High traffic volume
listed in the Candidate List of REACH Regulation
• Adjustable astragal
1907/2006/EC (date: 10.06.2022) exceeding 0.1 percentage by
Optional Features
mass: yes
• Battery backup for keeping the door operational during
• Lead (Pb):
power loss
7439-92-1 (CAS-No) is used in the steel alloy. The
• Various thresholds to fit any site condition
concentration of lead in the alloy does not exceed
• Bottom rail heights: 7-1/2", 10", and 12"
0,35% (by mass).
• Muntin bar widths: 6", 7", and 10"
• Transom Reference service life
• Crash bars The life cycle of the ESA 100-300 door system is about 10
• Glass stops up to 1"; sloped glass stops available years, depending on the application and frequency of use.
For placing on the market following standards are applicable: Regular maintenance is advised to ensure a life expectancy of
• ANSI A 156.10 10 years. For repairs or renewals, suitable spare parts are
• EN 16005 available. The drive is tested to 1,000,000 closing cycles
• ICC/IBC according to EN 16005.
• NFPA 70
• NFPA 101
• UL 325
Application
The ESA 100-300 are designed for interior or exterior
applications where emergency breakout of only the sliding
panels is required, The ESA 100-300 can be used for single
and double leaf doors.
Technical Data
The technical specification of the ESA 200 is as follows:
Constructional data
Name Value Unit
Height 240 mm
Installation depth 152 mm
Opening speed maximum 50 cm/s
Hold open time maximum 60 s
Supply voltage, frequency maximum 60 Hz
Power supply maximum 60 Hz
Internal power available 27 VDC/2A
Fuse 6.6 A
Power consumption maximum 250 W
Delivery status:The delivery status of an average ESA 200
automatic door system including header, drive, panels and
jambs and packaging is the following:
2 Environmental Product Declaration - Dormakaba - ESA 100-300 Automatic Sliding Door
LCA: Calculation rules
Declared Unit Use stage - Module B6
The declared unit is 1 piece of the product: ESA 100-300 The use stage related to the operation of the building includes:
Automatic Sliding Door — B6, operational energy use
Declared unit
End-of-life stage– Modules C1-C4 and D
Name Value Unit
The end-of-life stage includes:
Declared unit 1 pce.
— C1, de-construction, demolition:
Mass (total system) 209,43 kg — C2, transport to waste processing;
— C3, waste processing for reuse, recovery and/or recycling;
System boundary — C4, disposal;
The type of EPD is: cradle-to-gate with options, modules C1– including provision and all transport, provision of all materials,
C4, and module D (A1–A3 + C + D and additional modules: A4 products and related energy and water use.
+ A5 + B6)
Module D (Benefits and loads beyond the system boundary)
Production - Module A1-A3 includes:
The product stage includes: — D, recycling potentials, expressed as net impacts and
— A1, raw material extraction, processing and mechanical benefits.
treatments, processing of secondary material input (e.g.
Geographic Representativeness
recycling processes), — A2, transport to the manufacturer,
Land or region, in which the declared product system is
— A3, manufacturing and assembly including provision of all
manufactured, used or handled at the end of the product´s
materials, products and energy, as well as waste processing up
lifespan: Global
to the end-of-waste state.
Construction stage - Modules A4-A5
Comparability
The construction process stage includes:
Basically, a comparison or an evaluation of EPD data is only
— A4, transport to the building site;
possible if all the data sets to be compared were created
— A5, installation into the building;
according to EN 15804 and the building context, respectively
including provision of all materials, products and energy, as well
the product-specific characteristics of performance, are taken
as waste processing up to the end-of waste state or disposal of
into account. Background database: GaBi, SP40.
final residues during the construction process stage.
LCA: Scenarios and additional technical information
Reference service life
Characteristic product properties of biogenic carbon
Name Value Unit
Information on describing the Biogenic Carbon Content at
Life Span according to the manufacturer 10 a
factory gate
Name ValueUnit
kg
Biogenic carbon content in product 4.592
C Operational energy use (B6)
Biogenic carbon content in accompanying kg The use stage is declared for 10 years
0.736
packaging C Name Value Unit
Note: 1 kg of biogenic carbon is equivalent to 44/12 kg of CO . Electricity consumption for 1 year 189.29 kWh
2
Days per year in use 365 days
On mode per day 1.8 h
The following technical scenario information is required for the Idle mode per day 22.2 h
declared modules
On mode power 14,31 W
Transport from the gate to the site (A4)
Idle mode power 22.2 W
Name Value Unit
Litres of fuel (per 1 kg) 0.00276 l/100km
Capacity utilisation (including empty runs) 55 %
Transport distance via medium truck 100 km
Transport distance is declared for a distance of 100 km by truck
in order to allow scaling to a specific point of installation.
Installation into the building (A5)
Name Value Unit
Waste packaging (paper and plastic) 3 kg
3 Environmental Product Declaration - Dormakaba - ESA 100-300 Automatic Sliding Door
End of life (C1-C4)
Name Value Unit
Collected separately waste type 206.43 kg
Recycling 201 kg
Energy recovery 0.41 kg
Landfilling 5.02 kg
Transport to waste management 50 km
The product is disassembled in a recycling process.
Material recycling is then assumed for the metals and electronic
components. The plastic components are assumed to be
incinerated with energy recovery. Electromechanics and minor
proportions of residues arising from the recycling process are
landfilled.
Region for the End of Life is: Global.
Reuse, recovery and/or recycling potentials (D), relevant
scenario information
The collection rate is 100 %.
4 Environmental Product Declaration - Dormakaba - ESA 100-300 Automatic Sliding Door
LCA: Results
DESCRIPTION OF THE SYSTEM BOUNDARY (X = INCLUDED IN LCA; MND = MODULE OR INDICATOR NOT DECLARED; MNR
= MODULE NOT RELEVANT)
Benefits and
Construction loads beyond
Product stage Use stage End of life stage
process stage the system
boundaries
la ire ta m w a Ry lp p u s tro p s n a rT g n iru tc a fu n a M e h t m o rf tro p s n a rTe tis e h t o t e ta g y lb m e s s A e s U e c n a n e tn ia M ria p e R tn e m e c a lp e R tn e m h s ib ru fe R y g re n e la n o ita re p Oe s u re ta w la n o ita re p Oe s u n o itc u rts n o c -e Dn o itilo m e d tro p s n a rT g n is s e c o rp e ts a W la s o p s iD -e s u e R-y re v o c e R-g n ilc y c e Rla itn e to p
A1 A2 A3 A4 A5 B1 B2 B3 B4 B5 B6 B7 C1 C2 C3 C4 D
X X X X X MND MND MNR MNR MNR X MND MND X X X X
RESULTS OF THE LCA - ENVIRONMENTAL IMPACT according to EN 15804+A2: 1 piece ESA 100-300 Automatic Sliding Door
Parameter Unit A1-A3 A4 A5 B6 C2 C3 C4 D
GWP-total kg CO 2 eq 1.7E+03 1.83E+00 5.38E+00 1.06E+03 9.05E-01 2.49E+01 7.7E-02 -1.09E+03
GWP-fossil kg CO 2 eq 1.72E+03 1.75E+00 2.61E+00 1.06E+03 8.65E-01 1.39E+00 7.6E-02 -1.08E+03
GWP-biogenic kg CO 2 eq -2.14E+01 8.1E-02 2.77E+00 2.3E-01 4E-02 2.35E+01 2.6E-04 -3.53E+00
GWP-luluc kg CO 2 eq 1.59E+00 4.17E-05 1.9E-04 3.21E-01 2.06E-05 2.67E-04 2.19E-04 -1.63E-01
ODP kg CFC11 eq 1.76E-09 1.85E-16 1.79E-15 3.74E-12 9.13E-17 3.17E-15 2.82E-16 -8.94E-09
AP mol H+ eq 8.18E+00 2E-03 1E-03 1.72E+00 8.65E-04 3E-03 5.46E-04 -4.15E+00
EP-freshwater kg P eq 2.08E-03 3.75E-07 3.04E-07 5.81E-04 1.85E-07 4.75E-07 1.31E-07 -5.35E-04
EP-marine kg N eq 1.1E+00 5.58E-04 3.89E-04 3.68E-01 2.75E-04 1E-03 1.41E-04 -5.38E-01
EP-terrestrial mol N eq 1.2E+01 6E-03 6E-03 3.95E+00 3E-03 1.6E-02 2E-03 -5.85E+00
kg NMVOC
POCP 3.4E+00 2E-03 1E-03 1.05E+00 7.79E-04 3E-03 4.25E-04 -1.7E+00
eq
ADPE kg Sb eq 4.33E-03 5.25E-08 2.57E-08 2.11E-04 2.59E-08 4.91E-08 6.83E-09 -6.74E-04
ADPF MJ 2.24E+04 2.48E+01 2.07E+00 1.72E+04 1.23E+01 5.12E+00 9.98E-01 -1.56E+04
m3 world eq
WDP 2.6E+02 3E-03 6.12E-01 2.06E+02 2E-03 2.49E+00 8E-03 -4.7E+01
deprived
GWP = Global warming potential; ODP = Depletion potential of the stratospheric ozone layer; AP = Acidification potential of land and water; EP =
Eutrophication potential; POCP = Formation potential of tropospheric ozone photochemical oxidants; ADPE = Abiotic depletion potential for non-fossil
resources; ADPF = Abiotic depletion potential for fossil resources; WDP = Water (user) deprivation potential)
RESULTS OF THE LCA - INDICATORS TO DESCRIBE RESOURCE USE according to EN 15804+A2: 1 piece ESA 100-300
Automatic Sliding Door
Parameter Unit A1-A3 A4 A5 B6 C2 C3 C4 D
PERE MJ 9.45E+03 7.8E-02 2.45E+01 2.72E+03 3.9E-02 1.98E+02 1.31E-01 -7.59E+03
PERM MJ 2.21E+02 0 -2.4E+01 0 0 -1.97E+02 0 0
PERT MJ 9.67E+03 7.8E-02 4.69E-01 2.72E+03 3.9E-02 9.92E-01 1.31E-01 -7.59E+03
PENRE MJ 2.23E+04 2.49E+01 4.51E+01 1.72E+04 1.23E+01 2.85E+01 9.99E-01 -1.56E+04
PENRM MJ 6.64E+01 0 -4.3E+01 0 0 -2.34E+01 0 0
PENRT MJ 2.24E+04 2.49E+01 2.07E+00 1.72E+04 1.23E+01 5.12E+00 9.99E-01 -1.56E+04
SM kg 5.79E+00 0 0 0 0 0 0 0
RSF MJ 0 0 0 0 0 0 0 0
NRSF MJ 0 0 0 0 0 0 0 0
FW m3 2.38E+01 1.4E-04 1.4E-02 6.3E+00 6.94E-05 5.8E-02 2.52E-04 -1.32E+01
PERE = Use of renewable primary energy excluding renewable primary energy resources used as raw materials; PERM = Use of renewable primary
energy resources used as raw materials; PERT = Total use of renewable primary energy resources; PENRE = Use of non-renewable primary energy
excluding non-renewable primary energy resources used as raw materials; PENRM = Use of non-renewable primary energy resources used as raw
materials; PENRT = Total use of non-renewable primary energy resources; SM = Use of secondary material; RSF = Use of renewable secondary fuels;
NRSF = Use of non-renewable secondary fuels; FW = Use of net fresh water
RESULTS OF THE LCA – WASTE CATEGORIES AND OUTPUT FLOWS according to EN 15804+A2:
1 piece ESA 100-300 Automatic Sliding Door
Parameter Unit A1-A3 A4 A5 B6 C2 C3 C4 D
HWD kg 2.95E-05 2.41E-09 5.81E-09 6.63E-06 1.19E-09 5.1E-09 1.52E-08 -1.24E-05
NHWD kg 4.55E+02 3E-03 3.53E-01 5.35E+00 1E-03 2.64E-01 5.02E+00 -2.98E+02
RWD kg 1.36E+00 2.67E-05 9.08E-05 1.53E+00 1.32E-05 2.84E-04 1.14E-05 -1.79E+00
CRU kg 0 0 0 0 0 0 0 0
MFR kg 0 0 0 0 0 1.91E+02 0 0
MER kg 0 0 0 0 0 0 0 0
EEE MJ 0 0 9E+00 0 0 0 0 0
EET MJ 0 0 1.86E+01 0 0 0 0 0
5 Environmental Product Declaration - Dormakaba - ESA 100-300 Automatic Sliding Door
HWD = Hazardous waste disposed; NHWD = Non-hazardous waste disposed; RWD = Radioactive waste disposed; CRU = Components for re-use;
MFR = Materials for recycling; MER = Materials for energy recovery; EEE = Exported electrical energy; EET = Exported thermal energy
RESULTS OF THE LCA – additional impact categories according to EN 15804+A2-optional:
1 piece ESA 100-300 Automatic Sliding Door
Parameter Unit A1-A3 A4 A5 B6 C2 C3 C4 D
Disease
PM 8.53E-05 9.21E-09 1.02E-08 1.54E-05 4.55E-09 1.88E-08 6.76E-09 -6.73E-05
incidence
IR kBq U235 eq 2.71E+02 4E-03 1.1E-02 1.27E+02 2E-03 4.4E-02 1E-03 -3.64E+02
ETP-fw CTUe 7.94E+03 1.76E+01 8.67E-01 5.13E+03 8.69E+00 2.22E+00 5.7E-01 -5.95E+03
HTP-c CTUh 9.43E-07 3.31E-10 6.08E-11 1.1E-07 1.64E-10 1.63E-10 8.45E-11 -2.89E-07
HTP-nc CTUh 2.02E-05 1.42E-08 4.85E-09 4.17E-06 6.99E-09 6.63E-09 9.32E-09 -7.84E-06
SQP SQP 4.73E+03 6.4E-02 5.9E-01 1.57E+03 3.2E-02 1.44E+00 2.08E-01 -4.42E+02
PM = Potential incidence of disease due to PM emissions; IR = Potential Human exposure efficiency relative to U235; ETP-fw = Potential comparative
Toxic Unit for ecosystems; HTP-c = Potential comparative Toxic Unit for humans (cancerogenic); HTP-nc = Potential comparative Toxic Unit for humans
(not cancerogenic); SQP = Potential soil quality index
Disclaimer 1 – for the indicator IRP
This impact category deals mainly with the eventual impact of low dose ionizing radiation on human health of the nuclear fuel cycle. It
does not consider effects due to possible nuclear accidents, occupational exposure nor radioactive waste disposal in underground
facilities.Potential ionizing radiation from the soil, from radon and from some construction materials is also not measured by this
indicator.
Disclaimer 2 – for the indicators ADPE, ADPF, WDP, ETP-fw, HTP-c, HTP-nc, SQP
The results of this environmental impact indicator shall be used with care as the uncertainties on these results are high or as there is
limited experience with the indicator.
References
Standards EN 16005
DIN EN 16005: 2013-01, Power operated pedestrian doorsets -
A156.10 Safety in use - Requirements and test methods.
ANSI A156 - 2017 Power Operated Pedestrian Doors.
ICC/IBC
DIN 18650 The International Building Code (IBC) is a model building code
DIN 18650:2010, Powered pedestrian doors - Product developed by the International Code Council (ICC).
requirements and test methods. NFPA 70
National Electrical Code 70.
DIN EN 60335
DIN EN 60335-1, -2-103:2020-08, Household and similar NFPA 101
electrical appliances - Safety - Part 1: General requirements. Life Safety Code 101.
DIN EN 61000 UL 325
DIN EN 61000-1-2:2017-07, Electromagnetic compatibility UL 325:2017-05-19 Door, curtain, gate, blind and window
(EMC) - Part 1-2: General - Methodology for the achievement of operating devices and installations.
functional safety of electrical and electronic systems including
equipment with regard to electromagnetic phenomena. Further References
DIN EN 61508 2011/65/EU ROHS3 Directive
DIN EN 61508-2:2011-02, Functional safety of Directive 2011/65/EU of the European Parliament and of the
electrical/electronic/programmable electronic safety-related Council of 8 June 2011 on the restriction of the use of certain
systems - Part 2: Requirements for hazardous substances in electrical and electronic equipment.
electrical/electronic/programmable electronic safety-related IBU 2021
systems. General Instructions for the EPD programme of Institut Bauen
und Umwelt e.V.
DIN EN ISO 13849 Version 2.0, Berlin: Institut Bauen und Umwelt e.V., 2021.
DIN EN ISO 13849-1:2021-08, Safety of machinery - Safety- www.ibu-epd.com.
related parts of control systems - Part 1: General principles for
design. GaBi ts software
Sphera Solutions GmbH Gabi Software System and Database
DIN EN ISO 14025 for Life Cycle Engineering 1992-2020 Version 10.0.0.71
DIN EN ISO 14025:201110, Environmental labels and University of Stuttgart Leinfelden-Echterdingen.
declarations — Type III environmental declarations —
Principles and procedures. GaBi ts documentation
GaBi life cycle inventory data documentation
EN 15804 (https://www.gabisoftware.
EN 15804+A2: 2019+AC:2021, Sustainability of construction com/support/gabi/gabidatabase- 2020-lci-documentation/).
works — Environmental Product Declarations — Core rules for
the product category of construction products.
6 Environmental Product Declaration - Dormakaba - ESA 100-300 Automatic Sliding Door
LCA-tool dormakaba PCR Part B
LCA tool, version ENS Door LCA tool No.: IBU-DOR-202107- PCR – Part B: Requirements on the EPD for Building Hardware
LT1-EN Developed by Sphera Solutions GmbH. product, version 1.2, Institut Bauen und Umwelt e.V., www.ibu-
epd.com, 2020.
PCR Part A
PCR – Part A: Calculation Rules for the Life Cycle Assessment
and Requirements on the Project Re-port according to EN
15804+A2:2019, Version 1.0, Institut Bauen und Umwelt e.V.,
www.ibu-epd.com.
7 Environmental Product Declaration - Dormakaba - ESA 100-300 Automatic Sliding Door
Publisher
Institut Bauen und Umwelt e.V. +49 (0)30 3087748- 0
Hegelplatz 1 info@ibu-epd.com
10117 Berlin www.ibu-epd.com
Germany
Programme holder
Institut Bauen und Umwelt e.V. +49 (0)30 3087748- 0
Hegelplatz 1 info@ibu-epd.com
10117 Berlin www.ibu-epd.com
Germany
Author of the Life Cycle Assessment
Sphera Solutions GmbH +49 711 341817-0
Hauptstraße 111- 113 info@sphera.com
70771 Leinfelden-Echterdingen www.sphera.com
Germany
Owner of the Declaration
dormakaba International Holding GmbH +49 2333 793-0
DORMA Platz 1 info.de@dormakaba.com
58256 Ennepetal www.dormakaba.com
Germany
8 Environmental Product Declaration - Dormakaba - ESA 100-300 Automatic Sliding Door
