ENVIRONMENTAL-PRODUCT DECLARATION
as per ISO 14025 and EN 15804+A1
Owner of the Declaration Balsan Moquette
Publisher Institut Bauen und Umwelt e.V. (IBU)
Programme holder Institut Bauen und Umwelt e.V. (IBU)
Declaration number EPD-BAL-20210255-CCA3-EN
Issue date 27.11.2021
Valid to 26.11.2026
COLOR SCALE - GREY MATTERS - tufted carpet tiles/planks
Balsan
www.ibu-epd.com | https://epd-online.com
General Information
Balsan COLOR SCALE - GREY MATTERS - tufted carpet
tiles/planks
Programme holder Owner of the declaration
IBU – Institut Bauen und Umwelt e.V. Balsan Moquette
Hegelplatz 1 Corbilly 2
10117 Berlin 36330 Arthon
Germany France
Declaration number Declared product / declared unit
EPD-BAL-20210255-CCA3-EN 1 m² tufted carpet tiles or planks COLOR SCALE - GREY MATTERS.
This declaration is based on the product category rules: Scope:
Floor coverings, 01.08.2021 The manufacturer declaration applies to the tufted carpet tiles or planks
(PCR checked and approved by the SVR) COLOR SCALE - GREY MATTERS with the GUT-PRODIS license number
D47E97FA.
The products are produced in the Balsan manufacturing sites Arthon
Issue date (tufting and precoating) and Neuvy-Saint-Sépulchre (back coating),
France.
27.11.2021
The declaration is only valid in conjunction with a valid GUT-PRODIS
license of the product.
The owner of the declaration shall be liable for the underlying information
Valid to
and evidence; the IBU shall not be liable with respect to manufacturer
26.11.2026 information, life cycle assessment data and evidences.
The EPD was created according to the specifications of EN 15804+A1. In
the following, the standard will be simplified as EN 15804 bezeichnet.
Verification
The standard EN 15804 serves as the core PCR
Independent verification of the declaration and data according to ISO
14025:2011
internally X externally
Dipl.-Ing Hans Peters
(chairman of Institut Bauen und Umwelt e.V.)
Florian Pronold Angela Schindler,
(Managing Director Institut Bauen und Umwelt e.V.) (Independent verifier)
1 Environmental-Product Declaration - Balsan - COLOR SCALE - GREY MATTERS - tufted carpet tiles/planks
Product
Name Value Unit
Product description/Product definition
Polyamide 6 12.1 %
COLOR SCALE - GREY MATTERS - tufted carpet tiles or
Polyester 10.7 %
planks having a surface pile of solution-dyed polyamide 6 with
75% recycled content, a polyester primary backing with 100% SBR-latex 5.2 %
recycled content, a bitumen based heavy backing with a fibre Mineral filler 49.4 %
glass reinforcement and a fleece backing made of recycled Aluminum hydroxide 7.8 %
polyester.
Bitumen 13.9 %
The recycled content amounts to 19%. For the placing on the
Glass fibre 0.8 %
market of the product in the European Union/European Free
Trade Association (EU/EFTA) (with the exception of Additives 0.1 %
Switzerland) Regulation (EU) No. 305/2011 Construction This product contains substances listed in the ECHA candidate
Product Regulation (CPR) applies. The product needs a list (16.01.2020) or other carcinogenic, mutagenic or reprotoxic
Declaration of Performance (DoP) taking into (CMR) substances in categories 1A or 1B which are not on the
consideration EN 14041: 2018-05, Resilient, textile and candidate list exceeding 0.1 percentage by mass: no
laminate floor coverings - Essential characteristics, and the CE- The products are registered in the GUT-PRODIS Information
marking. The DoP of the product can be found on the System. The PRODIS system ensures the compliance with
manufacturer's technical information section. For the limitations of various chemicals and Volatile Organic Compound
application and use of the product the respective national (VOC)-emissions and a ban on the use of all substances that
provisions apply. are listed as 'Substances of Very High Concern' (SVHC) under
REACH.
Application
According to the use class as defined in EN 1307 the products
The main constituents of the product or its components shall be
can be used in all professional areas which require class 33 or
indicated as mass percentages to enable the user of the EPD
less.
to understand the composition of the product in delivery status.
This information should support safety and efficiency during
installation, use, and disposal of the product.
When substances from the “Candidate List of Substances of
Technical Data Very High Concern for Authorisation” (SVHC) are part of the
formulation with a mass percentage of > 0,1 of the mass of the
The performance data listed in the DoP apply.
construction product, i.e. when they were added to the
Name Value Unit
formulation on purpose, then the substances shall be declared
Tiles 50 cm x 50 cm or planks 100 cm x
Product Form - including CAS-number.
25 cm
Type of If the construction product is a substance or mixture under the
Tufted tiles -
manufacture chemical law (REACH), the concentration limit value refers to
Yarn type Polyamide 6, 75% recycled - the entire product; if it is an article, the partial product or
component applies as a unit of reference.
Coloration Solution dyed yarn
Primary backing Polyester, 100% recycled
The Candidate list can be found on the ECHA website address:
Secondary Bitumen based heavy backing with a - echa.europa.eu/de/home
backing recycled polyester felt
Total pile weight 500 g/m² This declaration is mandatory for all EPDs and must be
Surface pile formulated as follows:
220 g/m2
weight
1) “This product/article/at least one partial article contains
Total carpet
4145 g/m2 substances listed in the candidate list (date: dd.mm.yyyy)
weight
exceeding 0.1 percentage by mass: yes/no”.
Total thickness 9.2 mm
Performance data of the [if yes: List of respective SVHC and their CAS-number]
product in accordance with the declaration of performance with
respect Statements like “…free of ….” and/or “…does not contain…”
to its essential characteristics according to EN 14041: 2018- 05, may not be used.
Resilient, textile and laminate floor coverings - Essential
characteristics. Additional product properties in accordance with
Environment and health during use
EN 1307 can be found on the Product Information System
PRODIS using the PRODIS registration number of the product
Reference service life
(www.pro-dis.info) or on the manufacturer's technical
A calculation of the reference service life according to ISO
information section (www.balsan.com).
15686 is not possible.
Base materials/Ancillary materials The service life of textile floor coverings strongly depends on
the correct installation taking into account the declared use
classification and the adherence to cleaning and maintenance
instructions.
A minimum service life of 10 years can be assumed, technical
service life can be considerably longer.
2 Environmental-Product Declaration - Balsan - COLOR SCALE - GREY MATTERS - tufted carpet tiles/planks
LCA: Calculation rules
waste are listed in the result table as exported energy.
Declared Unit Biogenic carbon that is stored in renewable materials in
The declared unit and the mass reference must be indicated in packaging paper is released as carbon dioxide emissions into
the appropriate table as declared. If there are several units to the air at the end of life in module A5.
choose from, a suitable one must be selected. If averages are Preparation
declared across various products, the average breakdown must of the floor and auxiliary materials (adhesives, fixing agents,
be explained. PET
connectors) are beyond the system boundaries and not taken
1m² of floor covering with specified construction/composition into account.
parameters. The mass reference should be indicated. B1 Use:
Name Value Unit Indoor
Declared unit 1 m2 emissions during the use stage. After the first year, no
product-related Volatile Organic Compound (VOC) emissions
Gross density 450 kg/m3
are
The declared unit refers to 1 m2 produced textile floor covering. relevant due to known VOC decay curves of the product.
The output of module A5 'Assembly' is 1 m2 installed textile
floor covering. B2 Maintenance:
Cleaning of the textile floor covering for a period of 1 year:
For IBU core EPDs (where clause 3.6 is part of the EPD): for Vacuum cleaning – electricity supply
average EPDs, an estimate of the robustness of the LCA Wet cleaning – electricity, water consumption, production of the
values must be made, e.g. concerning variability of the cleaning agent, waste water treatment.
production process, geographical representativeness and the The
influence of background data and preliminary products declared values in this module have to be multiplied by the
compared to the environmental impacts caused by actual assumed
production. service life of the floor covering in the building in question.
B3 - B7:
The modules are not relevant and therefore not declared.
System boundary
Type of EPD: Cradle-to-grave C1 De-construction:
The floor covering is de-constructed manually and no additional
System boundaries of modules A, B, C, D: environmental impact is caused.
Modules C3, C4 and D are indicated separately for three end-
of-life scenarios: C2 Transport:
1 - landfill disposal Transport
2 - municipal waste incineration of the carpet waste to a landfill, to the municipal waste
3 - recovery in a cement plant incineration
A1-A3 Production: plant (MWI) or to the waste collection facility for recycling.
Energy
supply and production of the basic material, processing of C3 Waste processing:
secondary C3-1: Landfill disposal needs no waste processing.
material, auxiliary material, transport of the material to the C3-2: Impact from waste incineration (plant with
manufacturing site, emissions, waste water treatment, R1>0.6), generated electricity and steam are listed in the result
packaging material table as exported energy.
and waste processing up to the landfill disposal of residual C3-3: Collection of the carpet waste for recovery in the cement
waste industry, waste processing (granulating), transport to the
(except radioactive waste). Benefits for generated electricity cement plant, emissions from the incineration.
and steam
due to the incineration of production waste are aggregated. C4 Disposal
Biogenic carbon that is stored in renewable material (packaging C4-1: Impact from landfill disposal,
paper) is taken into account as well as the associated carbon C4-2: The carpet waste leaves the system in
dioxide uptake from the air from which this biogenic carbon module C3-2,
comes. C4-3: The pre-processed carpet waste leaves the system in
module C3-3.
A4 Transport:
Transport of the packed textile floor covering from factory gate D Recycling potential:
to the place of installation. Calculated benefits result from materials exclusive secondary
materials (net materials).
A5 Installation: D-A5: Benefits for generated energy due to incineration of
Installation packaging and installation waste (incineration plant with R1 >
of the textile floor covering, processing of installation waste and 0.6),
packaging waste up to the landfill disposal of residual waste D-1: Benefits for generated energy due to landfill disposal of
(except carpet waste at the end-of-life,
radioactive waste), the production of the amount of carpet that D-2: Benefits for generated energy due to incineration of carpet
occurs waste at the end-of-life (incineration plant with R1 > 0.6),
as installation waste including its transport to the place of D-3: Benefits for saved fossil energy and saved inorganic
installation. material due to recovery of the carpet in a cement plant.
Generated electricity and steam due to the incineration of
3 Environmental-Product Declaration - Balsan - COLOR SCALE - GREY MATTERS - tufted carpet tiles/planks
Geographic Representativeness Comparability
Land or region, in which the declared product system is Basically, a comparison or an evaluation of EPD data is only
manufactured, used or handled at the end of the product´s possible if all the data sets to be compared were created
lifespan: France according to EN 15804 and the building context, respectively
the product-specific characteristics of performance, are taken
into account.
LCA: Scenarios and additional technical information
conditions only.
The following information refer to the declared modules and are
the basis for calculations or can be used for further calculations. The same holds for a service life declared by the manufacturer.
Corresponding information related to in-use conditions needs
Transport to the construction site (A4)
not be provided if a service life taken from the list on service life
Name Value Unit
by BNB is declared.
Litres of fuel (truck, EURO 0-6 mix) 0.01 l/100km
Transport distance 700 km End of Life (C1-C4)
Capacity utilisation (including empty runs) 55 % Three different end-of-life scenarios are declared and the
Gross density of products transported 450 kg/m3 results are indicated separately in module C.
Each scenario is calculated as a 100% scenario.
Installation in the building (A5) Scenario 1: 100% landfill disposal
Name Value Unit Scenario 2: 100% municipal waste incineration (MWI)
with R1>0.6
Material loss 0.12 kg
Scenario 3: 100% recycling in the cement industry
Polyethylene packaging waste and installation waste are
considered to be incinerated in a municipal waste incineration If combinations of these scenarios have to be calculated this
plant. Cardboard is going to be recycled. should be done according to the following scheme:
Preparation of the floor and auxiliaries (adhesives, fixing EOL-impact = x% impact (Scenario 1)
agents, PET connectors etc.) are not taken into account. + y% impact (Scenario 2)
+ z% impact (Scenario 3)
Maintenance (B2) with x% + y% + z% = 100%
The values for cleaning refer to 1 m2 floor covering used in Name ValueUnit
commercial areas per year. Depending on the application Collected as mixed construction waste (scenario 1
4.145 kg
based on ISO 10874, the technical service life recommended and 2)
by the manufacturer and the anticipated strain on the floor by
Collected separately waste type (scenario 3) 4.145 kg
customers, the case- specific useful life can be established.
Landfilling (scenario 1) 4.145 kg
Based on this useful life the effects of Module B2 need to be
Energy recovery (scenario 2) 4.145 kg
calculated in order to obtain the overall environmental impacts.
Energy recovery (scenario 3) 1.738 kg
Name Value Unit
Recycling (scenario 3) 2.407 kg
Maintenance cycle (wet cleaning) 1.5 1/year
Maintenance cycle (vacuum cleaning) 208 1/year
Water consumption (wet cleaning) 0.004 m3 Reuse, recovery and/or recycling potentials (D), relevant
scenario information
Cleaning agent (wet cleaning) 0.09 kg
Recovery or recycling potentials due to the three end-of-life
Electricity consumption 0.314 kWh scenarios (module C) are indicated separately.
Further information on cleaning and maintenance see
www.balsan.com Recycling in the cement industry (scenario 3)
VDZ e.V.
The organic material of the carpet is used as secondary fuel in
In case a reference service life according to applicable ISO a cement kiln. It mainly substitutes for lignite (65.5%), hard coal
standards is declared then the assumptions and in-use (26.2%) and petrol coke (8.6%).
conditions underlying the determined RSL shall be declared. In The inorganic material is substantially integrated into the
addition, it shall be stated that the RSL applies for the reference cement clinker and substitutes for original material input.
4 Environmental-Product Declaration - Balsan - COLOR SCALE - GREY MATTERS - tufted carpet tiles/planks
LCA: Results
The declared result figures in module B2 have to be multiplied by the assumed service life (in years) of the floor covering in the building
under consideration.
Information on non-relevant modules: Modules B3 - B7 are not relevant during the service life of the carpet. Modules C1, C3/1, C4/2
and C4/3 cause no additional impact (see chapter "LCA: Calculation rules" in this document). All these modules are declared and
marked as 'modules not relevant/declared'. Module C2 represents the transport for scenarios 1, 2 and 3. Column D represents module
D/A5.
The calculations are based on the CML characterization factors (version August 2016).
DESCRIPTION OF THE SYSTEM BOUNDARY (X = INCLUDED IN LCA; MND = MODULE NOT DECLARED; MNR = MODULE NOT
RELEVANT)
BENEFITS
AND LOADS
CONSTRUCTION
BEYOND
PRODUCT STAGE PROCESS USE STAGE END OF LIFE STAGE
THE SYSTEM
STAGE
BOUNDARIE
S
la ire ta m w a Ry lp p u s tro p s n a rT g n iru tc a fu n a M e h t m o rf tro p s n a rTe tis e h t o t e ta g y lb m e s s A e s U e c n a n e tn ia M ria p e R tn e m e c a lp e R tn e m h s ib ru fe R y g re n e la n o ita re p Oe s u re ta w la n o ita re p Oe s u n o itc u rts n o c -e Dn o itilo m e d tro p s n a rT g n is s e c o rp e ts a W la s o p s iD -e s u e R-y re v o c e R-g n ilc y c e Rla itn e to p
A1 A2 A3 A4 A5 B1 B2 B3 B4 B5 B6 B7 C1 C2 C3 C4 D
X X X X X X X MNR MNR MNR MND MND MND X X X X
RESULTS OF THE LCA - ENVIRONMENTAL IMPACT according to EN 15804+A1: 1 m² floorcovering
Parameter Unit A1-A3 A4 A5 B1 B2 C2 C3/2 C3/3 C4/1 D D/1 D/2 D/3
GWP kg CO 2 eq 5.5E+00 2.46E-01 4.61E-01 0 2.92E-01 1.38E-02 4.61E+00 4.66E+00 2.82E-01 -1.68E-02 0 -5.1E-01 -2.9E-01
kg CFC11
ODP 2.32E-09 4.3E-17 6.97E-11 0 1.08E-08 2.4E-18 1.91E-15 2.64E-15 9.55E-16 -2.45E-16 0 -7.38E-15 -1.82E-15
eq
AP kg SO 2 eq 9.58E-03 1.02E-03 3.83E-04 0 1.08E-03 5.69E-05 2.11E-03 2.29E-03 7.3E-04 -1.89E-05 0 -5.71E-04 -9.91E-04
kg PO 3
EP 4 2.16E-02 2.59E-04 6.71E-04 0 3.02E-04 1.45E-05 5.07E-04 5.49E-04 7.93E-04 -2.63E-06 0 -7.94E-05 -1.43E-04
eq
kg Ethen
POCP 8.92E-04 -4.36E-04 1.68E-05 6.29E-05 1.45E-04 -2.44E-05 1.34E-04 7.65E-05 6.57E-05 -1.76E-06 0 -5.34E-05 -9.72E-05
eq
ADPE kg Sb eq 5.99E-06 2.18E-08 1.86E-07 0 2.74E-06 1.22E-09 1.8E-07 1.9E-07 5.4E-08 -3.05E-09 0 -9.21E-08 -1.86E-07
ADPF MJ 1.19E+02 3.35E+00 3.76E+00 0 6.76E+00 1.87E-01 2.49E+00 3.21E+00 4.2E+00 -2.44E-01 0 -7.41E+00 -2.92E+01
GWP = Global warming potential; ODP = Depletion potential of the stratospheric ozone layer; AP = Acidification potential of land and water; EP =
Eutrophication potential; POCP = Formation potential of tropospheric ozone photochemical oxidants; ADPE = Abiotic depletion potential for non-fossil
resources; ADPF = Abiotic depletion potential for fossil resources
RESULTS OF THE LCA - INDICATORS TO DESCRIBE RESOURCE USE according to EN 15804+A1: 1 m² floorcovering
Parameter Unit A1-A3 A4 A5 B1 B2 C2 C3/2 C3/3 C4/1 D D/1 D/2 D/3
PERE MJ 1.74E+01 1.87E-01 1.96E+00 0 1.23E+00 1.05E-02 4.54E-01 6.68E-01 3.14E-01 -6.32E-02 0 -1.9E+00 -4.28E-01
PERM MJ 1.38E+00 0 -1.38E+00 0 0 0 0 0 0 0 0 0 0
PERT MJ 1.87E+01 1.87E-01 5.82E-01 0 1.23E+00 1.05E-02 4.54E-01 6.68E-01 3.14E-01 -6.32E-02 0 -1.9E+00 -4.28E-01
PENRE MJ 1.06E+02 3.36E+00 4.36E+00 0 7.85E+00 1.88E-01 3.4E+01 3.49E+01 4.33E+00 -2.95E-01 0 -8.95E+00 -2.94E+01
PENRM MJ 3.13E+01 0 -4.3E-02 0 0 0 -3.13E+01 -3.13E+01 0 0 0 0 0
PENRT MJ 1.38E+02 3.36E+00 4.32E+00 0 7.85E+00 1.88E-01 2.75E+00 3.63E+00 4.33E+00 -2.95E-01 0 -8.95E+00 -2.94E+01
SM kg 9.08E-01 0 2.72E-02 0 0 0 0 0 0 0 0 0 1.39E+00
RSF MJ 0 0 0 0 0 0 0 0 0 0 0 0 0
NRSF MJ 0 0 0 0 0 0 0 0 0 0 0 0 0
FW m3 1.02E-01 2.15E-04 3.54E-03 0 4.13E-03 1.2E-05 1.52E-02 1.54E-02 3.99E-05 -6.17E-05 0 -1.86E-03 -2.71E-03
PERE = Use of renewable primary energy excluding renewable primary energy resources used as raw materials; PERM = Use of renewable primary
energy resources used as raw materials; PERT = Total use of renewable primary energy resources; PENRE = Use of non-renewable primary energy
excluding non-renewable primary energy resources used as raw materials; PENRM = Use of non-renewable primary energy resources used as raw
materials; PENRT = Total use of non-renewable primary energy resources; SM = Use of secondary material; RSF = Use of renewable secondary fuels;
NRSF = Use of non-renewable secondary fuels; FW = Use of net fresh water
RESULTS OF THE LCA – WASTE CATEGORIES AND OUTPUT FLOWS according to EN 15804+A1:
1 m² floorcovering
Parameter Unit A1-A3 A4 A5 B1 B2 C2 C3/2 C3/3 C4/1 D D/1 D/2 D/3
HWD kg 5.47E-06 1.69E-10 1.64E-07 0 5.9E-10 9.47E-12 4.97E-10 6.28E-10 7.79E-10 -6.57E-11 0 -1.99E-09 -3.84E-10
NHWD kg 3.1E-01 4.99E-04 4.52E-02 0 5.62E-03 2.79E-05 1.2E+00 1.2E+00 4.13E+00 -1.35E-04 0 -4.08E-03 -1.54E-01
RWD kg 7.4E-03 4.07E-06 2.25E-04 0 3.32E-04 2.27E-07 1.05E-04 1.66E-04 5.03E-05 -2.03E-05 0 -6.12E-04 -9.9E-05
CRU kg 0 0 0 0 0 0 0 0 0 0 0 0 0
MFR kg 8.62E-03 0 9.2E-02 0 0 0 0 1.39E+00 0 0 0 0 0
5 Environmental-Product Declaration - Balsan - COLOR SCALE - GREY MATTERS - tufted carpet tiles/planks
MER kg 0 0 0 0 0 0 0 0 0 0 0 0 0
EEE MJ 0 0 1.63E-01 0 0 0 5.21E+00 0 0 0 0 0 0
EET MJ 0 0 3.07E-01 0 0 0 9.84E+00 5.28E+01 0 0 0 0 0
HWD = Hazardous waste disposed; NHWD = Non-hazardous waste disposed; RWD = Radioactive waste disposed; CRU = Components for re-use;
MFR = Materials for recycling; MER = Materials for energy recovery; EEE = Exported electrical energy; EET = Exported thermal energy
Not all of the life cycle inventories applied in this study support the methodological approach for the waste and water indicators. The
data are based on publications of industry. The indicators for waste and water of the system are evaluated but contain a higher degree
of uncertainty.
References
EN 1307 No. 305/2011 Construction Products Regulation (CPR) of the
DIN EN 1307: 2014+A1:2016+A2:2018-05: Textile floor European
coverings - Classification Council and of the European Parliament, April 2011
EN 13501-1
DIN
EN 13501-1:2019-05: Fire classification of construction
products and CML characterization factors
building elements - Part 1: Classification using data from Impact assessment characterization factors, version 4.7,
reaction to August 2016, Institute of Environmental Sciences - 'Centrum
fire tests voor Milieuwetenschappen in Leiden' (CML), Leiden, The
EN 14041 Netherlands
DIN EN 14041: 2018-05: Resilient, textile and laminate floor
coverings - Essential characteristics
EN 15804
EN ECHA candidate list
15804:2012-04+A1 2013/, Sustainability of construction works
— Candidate List of substances of very high concern (SVHCs) for
Environmental Product Declarations — Core rules for the authorisation, 16.01.2020, European Chemicals Agency
product category (ECHA), Helsinki, Finland
of construction products
EN 16810
DIN
EN 16810: 2017-08: Resilient, textile and laminate floor ecoinvent 3.7
coverings –
Environmental product declarations – Product category rules ecoinvent, Zurich, Switzerland, database version 3.7, published
ISO 10874 September 2020
DIN EN ISO 10874: 2012+A1:2021-04: Resilient, textile and
laminate floor coverings - Classification
ISO 14025
DIN GaBi database 2021
EN /ISO 14025:2011-10/, Environmental labels and
declarations — Type GaBi Software-System and Database for Life Cycle
III environmental declarations — Principles and procedures Engineering, thinkstep AG, Leinfelden-Echterdingen, Database
release 2021-2
ISO 14040
DIN EN ISO 14040:2006+A1:2020 Environmental
management - Life cycle assessment - Principles and IBU 2021
framework
IBU
ISO 14044 (2021): General Programme Instructions for the Preparation of
DIN EN ISO 14044:2006+A1:2018+A2:2020 Environmental EPDs at
management - Life cycle assessment - Requirements and the Institut Bauen und Umwelt e.V., Version 2.0 Institut Bauen
guidelines und
ISO 15686 Umwelt e.V., Berlin. www.ibu-epd.de
ISO 15686: Buildings and constructed assets -
Service life planning
ISO 15686-1: 2011-05: Part 1: General principles and
framework PCR Part A
ISO 15686-2: 2012-05: Part 2: Service life prediction
procedures Product
ISO 15686-7: 2017-04: Part 7: Performance Category Rules for Construction Products from the range of
evaluation for feedback of service life data Environmental Product Declarations. Part A: Calculation Rules
from practice for the
ISO 15686-8: 2008-06: Part 8: Reference service life Life Cycle Assessment and Requirements on the Background
and service-life estimation Report, V1.9,
Regulation (EU) No. 305/2011 Berlin: Institut Bauen und Umwelt e.V. (IBU), January 2021
Regulation
6 Environmental-Product Declaration - Balsan - COLOR SCALE - GREY MATTERS - tufted carpet tiles/planks
PCR Part B REACH
Product Regulation
Category Rules for Construction Products from the range of (EC) No 1907/2006 of the European Parliament and of the
Environmental Product Declarations of Institut Bauen und Council of 18
Umwelt (IBU), December 2006 concerning the Registration, Evaluation,
Authorisation and
Part B: Requirements on the EPD for floor coverings, V1.2, Restriction of Chemicals (REACH). Last update: 27.02.2020
Berlin: Institut Bauen und Umwelt e.V. (IBU), February 2018 (Status:
27.06.2018)
PRODIS
VDZ e.V.
Product
Information System (PRODIS) of the European Carpet Industry, Association of German Cement Works, Ed. Environmental Data
Gemeinschaft umweltfreundlicher Teppichboden e.V (GUT) and of the German Cement Industry 2019
European The literature referred to in the Environmental Product
Carpet and Rug Association Declaration must be listed in full.Standards already fully quoted
in the EPD do not need to be listed here again.
(ECRA), http://www.pro-dis.info The current version of PCR Part A and PCR Part B of the PCR
document on which they are based must be referenced.
7 Environmental-Product Declaration - Balsan - COLOR SCALE - GREY MATTERS - tufted carpet tiles/planks
Publisher
Institut Bauen und Umwelt e.V. +49 (0)30 3087748- 0
Hegelplatz 1 info@ibu-epd.com
10117 Berlin www.ibu-epd.com
Germany
Programme holder
Institut Bauen und Umwelt e.V. +49 (0)30 3087748- 0
Hegelplatz 1 info@ibu-epd.com
10117 Berlin www.ibu-epd.com
Germany
Author of the Life Cycle Assessment
Gemeinschaft umweltfreundlicher Teppichboden +49 (0)241 96843 410
(GUT) e.V. mail@gut-ev.de
Schönebergstraße 2 www.gut-ev.org
52068 Aachen
Germany
Owner of the Declaration
Balsan Moquette +33 (0) 254 2916 00
Corbilly 2 cedric.charton@balsan.com
36330 Arthon www.balsan.com
France
8 Environmental-Product Declaration - Balsan - COLOR SCALE - GREY MATTERS - tufted carpet tiles/planks
