ENVIRONMENTAL PRODUCT DECLARATION
as per ISO 14025 and EN 15804+A2
Owner of the Declaration dormakaba International Holding GmbH
Publisher Institut Bauen und Umwelt e.V. (IBU)
Programme holder Institut Bauen und Umwelt e.V. (IBU)
Declaration number EPD-DOR-20220260-CBA1-EN
Issue date 29.11.2022
Valid to 28.11.2027
EL 301 Series Sliding Door Operator
Dormakaba
www.ibu-epd.com | https://epd-online.com
General Information
Dormakaba EL 301 Series Sliding Door Operator
Programme holder Owner of the declaration
IBU – Institut Bauen und Umwelt e.V. dormakaba International Holding GmbH
Hegelplatz 1 DORMA Platz 1
10117 Berlin 58256 Ennepetal
Germany Germany
Declaration number Declared product / declared unit
EPD-DOR-20220260-CBA1-EN 1 piece of the product: EL 301 Series - sliding door operator, consisting of
the following items:
- EL 301 profiles
- EL 301 drive components, consisting of motor, controller, power supply
- EL 301 belt drive components
- EL 301 accesssories battery pack and lock
- EL301 carrier components
- additional mechanical components
- packaging
This declaration is based on the product category rules: Scope:
Drive systems for automatic doors and gates, 01.08.2021 This EPD refers to a specific automatic sliding door operator EL 301 series
(PCR checked and approved by the SVR) produced by dormakaba. The production site is located in Hallam,
Australia. The material and energy flows were taken into consideration
accordingly.
Issue date
The year of data collection is 2022.
29.11.2022
The owner of the declaration shall be liable for the underlying information
and evidence; the IBU shall not be liable with respect to manufacturer
information, life cycle assessment data and evidences.
Valid to
28.11.2027 The EPD was created according to the specifications of EN 15804+A2. In
the following, the standard will be simplified as EN 15804.
Verification
The standard EN 15804 serves as the core PCR
Independent verification of the declaration and data according to ISO
14025:2011
internally X externally
Dipl.-Ing. Hans Peters
(Chairman of Institut Bauen und Umwelt e.V.)
Florian Pronold Dr.-Ing. Wolfram Trinius,
(Managing Director Institut Bauen und Umwelt e.V.) (Independent verifier)
1 Environmental Product Declaration - Dormakaba - EL 301 Series Sliding Door Operator
Product
Product description/Product definition Delivery status:
The dormakaba EL 301 automatic door operator is engineered
to control and operate bi-parting and single slide framed and The declared EL301 series sliding door operator includes the
frameless glass sliding doors. profiles, drive, belt drive, carrier, battery pack and lock,
mechanical components and packaging with a weight of 73,14
Features kg.
• Total door weight to 300 kg
• Made In Australia
• Integrated uninterruptible power supply (UPS) system
• Smart lock technology
For the placing on the market the following legal provisions
apply:
• Australian Standard AS5007
Base materials/Ancillary materials
• Endurance
The EL 301 automatic sliding door operator comprises the
testing clause 4.4.1.1. and 4.4.2 by NATA
following components including packaging:
accredited facility.
• 2011/65/EU ROHS3 Directive
Application
The dormakaba EL 301 automatic door operator is a proven
performer in airports, shopping centres, supermarkets, hotels,
hospitals, financial institutions, sports stadiums and many other
commercial sites.
The following parameter are applicable for single and double-
leaf doors:
Single-panel sliding door
· Maximum door width: 3000 mm
· Maximum door weight: 300 kg
Double leaf sliding door
· Maximum door width: 1500 mm The product contains partial articles which contain substances
· Maximum door weight: 150 kg listed in the Candidate List of REACH
Regulation 1907/2006/EC (date: 10.06.2022) exceeding 0.1
Technical Data
percentage by mass: yes
The technical data of the EL 301 are as follows:
• Lead (Pb):
Constructional data
7439-92-1 (CAS-No) is used in the brass alloy. The
Name Value Unit concentration of lead in the alloy does not exceed
Height 240 mm 4%(by mass).
Installation depth 152 mm • The drive system is battery-powered (lead accumulator).
Opening speed maximum 50 cm/s
Reference service life
Closing speed maximum 40 cm/s The life cycle of the EL 301 series is about 10 years, depending
Hold open time maximum 60 s on the application and frequency of use. Regular maintenance
Supply voltage, frequency maximum 60 Hz is advised to ensure the life expectancy of 10 years. For repairs
or renewals, suitable spare parts are available. The EL 301 is
Power consumption 175 W
tested and certified to 1,000,000 cycles according to AS 5007
Class of protection 20 IP
NATA accredited.
Product in accordance with:
• Australian Standard AS5007
LCA: Calculation rules
Declared Unit System boundary
The declared unit is 1 piece of the product: EL 301 Series The type of EPD is: cradle-to-gate with options, modules C1–
Sliding Door Operator C4, and module D (A1–A3 + C + D and additional modules: A4
+ A5 + B6)
Declared unit
Name Value Unit
Production - Module A1-A3
Declared unit 1 pce. The product stage includes:
Mass (total system) (excl. packaging) 73,14 kg — A1, raw material extraction, processing and mechanical
treatments, processing of secondary material input (e.g.
recycling processes), — A2, transport to the manufacturer,
2 Environmental Product Declaration - Dormakaba - EL 301 Series Sliding Door Operator
— A3, manufacturing and assembly including provision of all — C4, disposal;
materials, products and energy, as well as waste processing up including provision and all transport, provision of all materials,
to the end-of waste state. products and related energy and water use.
Construction stage - Modules A4-A5 Module D (Benefits and loads beyond the system boundary)
The construction process stage includes: includes:
— A4, transport to the building site; — D, recycling potentials, expressed as net impacts and
— A5, installation into the building; benefits.
including provision of all materials, products and energy, as well
as waste processing up to the end-of waste state or disposal of Geographic Representativeness
final residues during the construction process stage. Land or region, in which the declared product system is
manufactured, used or handled at the end of the product´s
Use stage - Module B6 lifespan: Australia
The use stage related to the operation of the building includes:
— B6, operational energy use
Comparability
Basically, a comparison or an evaluation of EPD data is only
End-of-life stage– Modules C1-C4 and D
possible if all the data sets to be compared were created
The end-of-life stage includes:
according to EN 15804 and the building context, respectively
— C1, de-construction, demolition:
the product-specific characteristics of performance, are taken
— C2, transport to waste processing;
into account. Background database: GaBi, SP40.
— C3, waste processing for reuse, recovery and/or recycling;
LCA: Scenarios and additional technical information
Characteristic product properties of biogenic carbon
Information on describing the Biogenic Carbon Content at Operational energy use (B6)
factory gate The use stage is declared for 10 years
Name ValueUnit Name Value Unit
Biogenic carbon content in product 0.18 kg Electricity consumption for 1 year 93.84 kWh
C
Days per year in use 365 days
Biogenic carbon content in accompanying kg
0.52 On mode per day 1 h
packaging C
Idle mode per day 7 h
Note: 1 kg of biogenic carbon is equivalent to 44/12 kg of CO .
2 Off mode per day 16 h
On mode power 67,2 W
Idle mode power 7,7 W
The following technical scenario information is required for the
declared modules Off mode power 8,5 W
Transport from the gate to the site (A4) End of life (C1-C4)
Name Value Unit Name Value Unit
Litres of fuel (per 1 kg) 0.00276 l/100km Recycling 67.9 kg
Capacity utilisation (including empty runs) 55 % Energy recovery 1.27 kg
Transport distance via medium truck 100 km Landfilling 2.58 kg
Transport distance is declared for a distance of 100km by truck Transport to waste management 50 km
in order to allow scaling to a specific point of installation.
The product is disassembled in a recycling process.
Material recycling is then assumed for the metals, electronics
Installation into the building (A5) and electromechanics. The plastic components are assumed to
Name Value Unit be incinerated with energy recovery. Minor proportions of
residues arising from the recycling process are landfilled.
Waste packaging (paper and plastic) 1.42 kg
Region for the End of Life is: Global.
Reference service life
Reuse, recovery and/or recycling potentials (D), relevant
Name Value Unit
scenario information
Life Span according to the manufacturer 10 a
The collection rate is 100 %.
3 Environmental Product Declaration - Dormakaba - EL 301 Series Sliding Door Operator
LCA: Results
DESCRIPTION OF THE SYSTEM BOUNDARY (X = INCLUDED IN LCA; MND = MODULE OR INDICATOR NOT DECLARED; MNR
= MODULE NOT RELEVANT)
Benefits and
Construction loads beyond
Product stage Use stage End of life stage
process stage the system
boundaries
la ire ta m w a Ry lp p u s tro p s n a rT g n iru tc a fu n a M e h t m o rf tro p s n a rTe tis e h t o t e ta g y lb m e s s A e s U e c n a n e tn ia M ria p e R tn e m e c a lp e R tn e m h s ib ru fe R y g re n e la n o ita re p Oe s u re ta w la n o ita re p Oe s u n o itc u rts n o c -e Dn o itilo m e d tro p s n a rT g n is s e c o rp e ts a W la s o p s iD -e s u e R-y re v o c e R-g n ilc y c e Rla itn e to p
A1 A2 A3 A4 A5 B1 B2 B3 B4 B5 B6 B7 C1 C2 C3 C4 D
X X X X X MND MND MNR MNR MNR X MND X X X X X
RESULTS OF THE LCA - ENVIRONMENTAL IMPACT according to EN 15804+A2: 1 piece EL 301 Sliding Door Operator
Parameter Unit A1-A3 A4 A5 B6 C1 C2 C3 C4 D
GWP-total kg CO 2 eq 5.31E+02 6.4E-01 2.02E+00 9.42E+02 0 3.11E-01 4.3E+00 1.31E-01 -2.78E+02
GWP-fossil kg CO 2 eq 5.33E+02 6.11E-01 6.3E-02 9.41E+02 0 2.98E-01 3.23E+00 1.3E-01 -2.77E+02
GWP-biogenic kg CO 2 eq -2.7E+00 2.8E-02 1.96E+00 8.46E-01 0 1.4E-02 1.07E+00 4.44E-04 -8.52E-01
GWP-luluc kg CO 2 eq 3.85E-01 1.46E-05 3.38E-05 2.25E-01 0 7.08E-06 1.89E-04 3.74E-04 -4.1E-02
ODP kg CFC11 eq 3.74E-09 6.46E-17 3.68E-16 4.3E-12 0 3.14E-17 1.71E-15 4.82E-16 -2.07E-09
AP mol H+ eq 2.72E+00 6.12E-04 5.65E-04 4.52E+00 0 2.98E-04 6.91E-04 9.33E-04 -1.22E+00
EP-freshwater kg P eq 7.18E-04 1.31E-07 7.18E-08 4.38E-04 0 6.37E-08 2.72E-07 2.23E-07 -1.39E-04
EP-marine kg N eq 3.68E-01 1.95E-04 2.04E-04 9.67E-01 0 9.48E-05 1.6E-04 2.4E-04 -1.46E-01
EP-terrestrial mol N eq 4.01E+00 2E-03 3E-03 1.06E+01 0 1E-03 3E-03 3E-03 -1.58E+00
kg NMVOC
POCP 1.15E+00 5.51E-04 5.4E-04 2.69E+00 0 2.68E-04 4.44E-04 7.27E-04 -4.71E-01
eq
ADPE kg Sb eq 2.35E-02 1.83E-08 5.8E-09 6.31E-05 0 8.93E-09 2.37E-08 1.17E-08 -1.2E-02
ADPF MJ 6.77E+03 8.67E+00 6.4E-01 1.04E+04 0 4.22E+00 1.65E+00 1.71E+00 -3.88E+03
m3 world eq
WDP 8.11E+01 1E-03 2.5E-01 3.57E+02 0 5.83E-04 4.28E-01 1.4E-02 -1.42E+01
deprived
GWP = Global warming potential; ODP = Depletion potential of the stratospheric ozone layer; AP = Acidification potential of land and water; EP =
Eutrophication potential; POCP = Formation potential of tropospheric ozone photochemical oxidants; ADPE = Abiotic depletion potential for non-fossil
resources; ADPF = Abiotic depletion potential for fossil resources; WDP = Water (user) deprivation potential)
RESULTS OF THE LCA - INDICATORS TO DESCRIBE RESOURCE USE according to EN 15804+A2: 1 piece EL 301 Sliding Door
Operator
Parameter Unit A1-A3 A4 A5 B6 C1 C2 C3 C4 D
PERE MJ 2.4E+03 2.7E-02 1.71E+01 1.59E+03 0 1.3E-02 1.3E+01 2.24E-01 -1.76E+03
PERM MJ 2.96E+01 0 -1.7E+01 0 0 0 -1.26E+01 0 0
PERT MJ 2.43E+03 2.7E-02 1.17E-01 1.59E+03 0 1.3E-02 4.18E-01 2.24E-01 -1.76E+03
PENRE MJ 6.74E+03 8.68E+00 8.55E-01 1.04E+04 0 4.22E+00 3.78E+01 1.71E+00 -3.88E+03
PENRM MJ 3.63E+01 0 -2.15E-01 0 0 0 -3.61E+01 0 0
PENRT MJ 6.78E+03 8.68E+00 6.4E-01 1.04E+04 0 4.22E+00 1.65E+00 1.71E+00 -3.88E+03
SM kg 4.53E+00 0 0 0 0 0 0 0 0
RSF MJ 0 0 0 0 0 0 0 0 0
NRSF MJ 0 0 0 0 0 0 0 0 0
FW m3 6.03E+00 4.9E-05 6E-03 5.01E+00 0 2.39E-05 1E-02 4.3E-04 -3.16E+00
PERE = Use of renewable primary energy excluding renewable primary energy resources used as raw materials; PERM = Use of renewable primary
energy resources used as raw materials; PERT = Total use of renewable primary energy resources; PENRE = Use of non-renewable primary energy
excluding non-renewable primary energy resources used as raw materials; PENRM = Use of non-renewable primary energy resources used as raw
materials; PENRT = Total use of non-renewable primary energy resources; SM = Use of secondary material; RSF = Use of renewable secondary fuels;
NRSF = Use of non-renewable secondary fuels; FW = Use of net fresh water
RESULTS OF THE LCA – WASTE CATEGORIES AND OUTPUT FLOWS according to EN 15804+A2:
1 piece EL 301 Sliding Door Operator
Parameter Unit A1-A3 A4 A5 B6 C1 C2 C3 C4 D
HWD kg 1.51E-05 8.42E-10 9.57E-10 1.69E-06 0 4.1E-10 5.8E-09 2.6E-08 -2.13E-05
NHWD kg 1.15E+02 8.87E-04 6.4E-02 2.69E+00 0 4.32E-04 3.4E-01 8.58E+00 -6.9E+01
RWD kg 3.61E-01 9.32E-06 3.35E-05 2E-03 0 4.53E-06 6.46E-05 1.94E-05 -4.2E-01
CRU kg 0 0 0 0 0 0 0 0 0
MFR kg 0 0 0 0 0 0 6.11E+01 0 0
MER kg 0 0 0 0 0 0 0 0 0
EEE MJ 0 0 3.06E+00 0 0 0 0 0 0
EET MJ 0 0 5.56E+00 0 0 0 0 0 0
4 Environmental Product Declaration - Dormakaba - EL 301 Series Sliding Door Operator
HWD = Hazardous waste disposed; NHWD = Non-hazardous waste disposed; RWD = Radioactive waste disposed; CRU = Components for re-use;
MFR = Materials for recycling; MER = Materials for energy recovery; EEE = Exported electrical energy; EET = Exported thermal energy
RESULTS OF THE LCA – additional impact categories according to EN 15804+A2-optional:
1 piece EL 301 Sliding Door Operator
Parameter Unit A1-A3 A4 A5 B6 C1 C2 C3 C4 D
Disease
PM 2.89E-05 3.22E-09 3.14E-09 4.6E-05 0 1.57E-09 7.97E-09 1.16E-08 -1.78E-05
incidence
IR kBq U235 eq 6.81E+01 1E-03 5E-03 2.53E-01 0 6.48E-04 6E-03 2E-03 -8.45E+01
ETP-fw CTUe 2.45E+03 6.15E+00 3.03E-01 1.43E+03 0 2.99E+00 6.31E-01 9.75E-01 -1.41E+03
HTP-c CTUh 2.95E-07 1.16E-10 1.61E-11 8.4E-08 0 5.63E-11 5.5E-11 1.45E-10 -6.1E-08
HTP-nc CTUh 7.09E-06 4.94E-09 7.09E-10 3.09E-06 0 2.41E-09 5.12E-09 1.59E-08 -1.92E-06
SQP SQP 1.12E+03 2.2E-02 1.7E-01 9.75E+02 0 1.1E-02 4.92E-01 3.56E-01 -1.19E+02
PM = Potential incidence of disease due to PM emissions; IR = Potential Human exposure efficiency relative to U235; ETP-fw = Potential comparative
Toxic Unit for ecosystems; HTP-c = Potential comparative Toxic Unit for humans (cancerogenic); HTP-nc = Potential comparative Toxic Unit for humans
(not cancerogenic); SQP = Potential soil quality index
Disclaimer 1 – for the indicator IRP
This impact category deals mainly with the eventual impact of low dose ionizing radiation on human health of the nuclear fuel cycle. It
does not consider effects due to possible nuclear accidents, occupational exposure nor radioactive waste disposal in underground
facilities. Potential ionizing radiation from the soil, from radon and from some construction materials is also not measured by this
indicator.
Disclaimer 2 – for the indicators ADPE, ADPF, WDP, ETP-fw, HTP-c, HTP-nc, SQP
The results of this environmental impact indicator shall be used with care as the uncertainties on these results are high or as there is
limited experience with the indicator.
References
Standards University of Stuttgart Leinfelden-Echterdingen
AS 5007 GaBi ts documentation
AS 5007-2007 Powered doors for pedestrian access and GaBi life cycle inventory data documentation
egress (https://www.gabisoftware.
com/support/gabi/gabidatabase- 2020-lci-documentation/).
ISO 14025
DIN EN ISO 14025:201110, Environmental labels and LCA-tool dormakaba
declarations — Type III environmental declarations — LCA tool, ENS (drive system) LCA tool no.: IBU-DOR-202108-
Principles and procedures LT1-EN Developed by Sphera Solutions GmbH.
Further References PCR Part A
2011/65/EU ROHS3 Directive PCR – Part A: Calculation Rules for the Life Cycle Assessment
Directive 2011/65/EU of the European Parliament and of the and Requirements on the Project Re-port according to EN
Council of 8 June 2011 on the restriction of the use of certain 15804+A2:2019, Version 1.0, Institut Bauen und Umwelt e.V.,
hazardous substances in electrical and electronic equipment www.ibu-epd.com.
IBU 2021
General Instructions for the EPD programme of Institut Bauen PCR Part B
und Umwelt e.V. PCR – Part B: Requirements on the EPD for Building Hardware
Version 2.0, Berlin: Institut Bauen und Umwelt e.V., 2021. product, version 1.2, Institut Bauen und Umwelt e.V., www.ibu-
www.ibu-epd.com epd.com, 2020.
GaBi ts software
Sphera Solutions GmbH Gabi Software System and Database
for Life Cycle Engineering 1992-2020 Version 10.0.0.71
5 Environmental Product Declaration - Dormakaba - EL 301 Series Sliding Door Operator
Publisher
Institut Bauen und Umwelt e.V. +49 (0)30 3087748- 0
Hegelplatz 1 info@ibu-epd.com
10117 Berlin www.ibu-epd.com
Germany
Programme holder
Institut Bauen und Umwelt e.V. +49 (0)30 3087748- 0
Hegelplatz 1 info@ibu-epd.com
10117 Berlin www.ibu-epd.com
Germany
Author of the Life Cycle Assessment
Sphera Solutions GmbH +49 711 341817-0
Hauptstraße 111- 113 info@sphera.com
70771 Leinfelden-Echterdingen www.sphera.com
Germany
Owner of the Declaration
dormakaba International Holding GmbH +49 2333 793-0
DORMA Platz 1 info.de@dormakaba.com
58256 Ennepetal www.dormakaba.com
Germany
6 Environmental Product Declaration - Dormakaba - EL 301 Series Sliding Door Operator
