Environmental Product Declaration (EPD)
According to ISO 14025 and EN 15804
ACETex® PP
Registration number: EPD-Kiwa-EE-158058-EN
Issue date: 22-12-2023
Valid until: 22-12-2028
Declaration owner: Gold-Joint Industry Co., Ltd.
Publisher: Kiwa-Ecobility Experts
Program operator: Kiwa-Ecobility Experts
Status: verified
ACETex® PP | ReTHiNK-58058 1 / 25
Environmental Product Declaration
1 General information
E-mail: marketing@geoace.com
1.1 PRODUCT Website: www.geoace.com
Production location: Gold-Joint Industry Co., Ltd.
ACETex® PP
Address production location: No.33, Jing 3 Rd. Wuqi Dist., 43541 Taichung City
1.2 REGISTRATION NUMBER
1.6 VERIFICATION OF THE DECLARATION
EPD-Kiwa-EE-158058-EN
The independent verification is in accordance with the ISO 14025:2011. The LCA is in
1.3 VALIDITY compliance with ISO 14040:2006 and ISO 14044:2006. The EN 15804:2012+A2:2019 serves as
the core PCR.
Issue date: 22-12-2023
Internal ✓ External
Valid until: 22-12-2028
1.4 PROGRAM OPERATOR
Kiwa-Ecobility Experts
Voltastraße 5
13355 Berlin
DE
Elisabeth Amat Guasch, Greenize
1.7 STATEMENTS
Prof. Dr. Frank Heimbecher
The owner of this EPD shall be liable for the underlying information and evidence. The
(Chairman of the independent expert
programme operator Kiwa-Ecobility Experts shall not be liable with respect to
committee - Kiwa-Ecobility Experts)
manufacturer data, life cycle assessment data and evidence.
Frank Huppertz 1.8 PRODUCT CATEGORY RULES
(Head of Kiwa-Ecobility Experts)
Kiwa-Ecobility Experts (Kiwa-EE) – General Product Category Rules (2022-02-14)
Kiwa-Ecobility Experts (Kiwa-EE) – Specific Product Category Rules: Geosynthetic products
1.5 OWNER OF THE DECLARATION
(2023-07-21)
Manufacturer: Gold-Joint Industry Co., Ltd.
Address: No.33, Jing 3 Rd. Wuqi Dist., 43541 Taichung City, Taiwan (R.O.C.)
ACETex® PP | ReTHiNK-58058 2 / 25
Environmental Product Declaration
1 General information
1.9 COMPARABILITY 1.10 CALCULATION BASIS
In principle, a comparison or assessment of the environmental impacts of different LCA method R<THiNK: Ecobility Experts | EN15804+A2
products is only possible if they have been prepared in accordance with EN 15804. For the
evaluation of the comparability, the following aspects have to be considered in particular: LCA software*: Simapro 9.1
PCR used, functional or declared unit, geographical reference, the definition of the system Characterization method: EN 15804 +A2 Method v1.0
boundary, declared modules, data selection (primary or secondary data, background
database, data quality), scenarios used for use and disposal phases, and the life cycle LCA database profiles: EcoInvent version 3.6
inventory (data collection, calculation methods, allocations, validity period). PCRs and Version database: v3.15 (2023-07-12)
general program instructions of different EPDs programs may differ. Comparability needs
to be evaluated. For further guidance, see EN 15804+A2 (5.3 Comparability of EPD for
*Used for calculating the characterized results of the Environmental profiles within
construction products) and ISO 14025 (6.7.2 Requirements for comparability).
R<THiNK.
1.11 LCA BACKGROUND REPORT
This EPD is generated on the basis of the LCA background report 'ACETex® PP' with the
calculation identifier ReTHiNK-58058.
ACETex® PP | ReTHiNK-58058 3 / 25
Environmental Product Declaration
2 Product
2.1 PRODUCT DESCRIPTION
ACETex® PP is a high-performance woven geotextile that caters to the integrated
engineering demands of strength, filtration, and separation. The ACETex® PP woven
geotextile is manufactured using patented PP industrial yarn, endowing ACETex® PP with
high strength and excellent permeability under appropriate opening sizes. Through in-
house testing and verification by professional third-party laboratories, ACETex® PP has
been proven to possess exceptional durability, including resistance to oxidation, UV,
abrasion, chemicals, and biodegradation. ACETex® PP is suitable for various applications,
ranging from surface erosion control, separation, and filtration of drainage systems, to
being processed into geotextile tubes.
The following products are covered in this EPD: GT40-II PP, GT50-II PP, GT60-II PP, GT70-II
PP, GT70-I PP / GT70-I TA, GT80-II PP, GT100-II PP, GT120-II PP, GT130-II PP, GT175-II PP,
GT200-II PP / GT200-II TA, GT250-II PP.
2.2 APPLICATION (INTENDED USE OF THE PRODUCT)
ACETex® PP woven geotextiles, made from high-tenacity polypropylene yarns, serve
various engineering purposes with their demonstrated abilities in separation, filtration, and
reinforcement. In road construction, the material is particularly valued for its role in
stabilizing subgrades. Engineers are examining its potential contributions to reducing
ACETex® PP | ReTHiNK-58058 4 / 25
Environmental Product Declaration
2 Product
rutting and extending the service life of roads. ACETex® PP is also relevant in subgrade
stabilization projects where challenging soil conditions exist. With the increasing
frequency of extreme weather events, the material's capabilities in water management
and soil retention are subjects of ongoing research for ensuring long-term structural
integrity. In addition, ACETex® PP is utilized in fabricating specialized products such as
geotextile tubes and bags, which require both high tensile strength and effective
permeability for efficient filling and dewatering processes.
2.3 REFERENCE SERVICE LIFE
RSL PRODUCT
According to the application standard (EN 13249–13257, EN 13265, and EN 15381), the typical
RSL of ACETex® PP is about 50 years.
USED RSL (YR) IN THIS LCA CALCULATION:
2.7 CONSTRUCTION DESCRIPTION
50
The geotextile construction can be divided into the following parts:
2.4 TECHNICAL DATA
-Site preparation
See above (2.1).
-Geotextile installation
-Backfill and compaction
2.5 SUBSTANCES OF VERY HIGH CONCERN
The product contains less than 0.1% of substances included in the “Candidate list of
substances of very high concern for authorisation” (SVHC).
2.6 DESCRIPTION PRODUCTION PROCESS
The foundational material for manufacturing ACETex® PP woven geotextile is PP yarn.
Most of this PP yarn is produced in-house, while a portion is purchased externally. Before
weaving, some of the PP yarn needs to be twisted into processed yarn, while other batches
don’t require this step. This operation is carried out both by our team and external
collaborators.
Once the warp yarn is either warped or directly placed on the yarn creel, the weaving
process can commence. Weaving, a method of fabric production, involves interlacing two
distinct sets of yarn at right angles. These sets of yarns run in a longitudinal warp direction
(machine direction) and a transversal weft direction (cross-machine direction),
respectively. Once the weaving is completed, the fabric is wound onto a cloth beam and
transported to the next station for visual inspection. After confirmation of its quality, the
fabric is wound onto paper tubes at required lengths, packaged, and then stored in the
warehouse.
ACETex® PP | ReTHiNK-58058 5 / 25
Environmental Product Declaration
2 Product
ACETex® PP | ReTHiNK-58058 6 / 25
Environmental Product Declaration
3 Calculation rules
31.D ECLARED UNIT Module B2 = Maintenance Module C4 = Disposal
Module D = Benefits and loads beyond the
One square meter ACETex® PP Module B3 = Repair
product system boundaries
One square meter of ACETex® PP. The following products are T4co0v-eIIr ed in this EPD: G
Module B4 = Replacement
PP, GT50-II PP, GT60-II PP, GT70-II PP, GT70-I PP / GT70-I TA, GT80-II PP, GT100-II PP,
GT120-II PP, GT130-II PP, GT1G75T-II 2PP,0 0-II PP / GT200-II TA, GT250-II PP.
reference_unit: square meter (m2) 3.4 REPRESENTATIVENESS
The input data are representative for AceTex® PP , a product of Gold-Joint Industry.
32.C ONVERSION FACTORS
The data are representative for Asia.
Description Value Unit
3.C5U T-OFF CRITERIA
reference_unit 1 m2
weight_per_reference_unit 1.318 kg Product Stage (1A -A3)
Conversion factor to 1 kg 0.758668 m2
The following input have been placed under cut-off criteria (<1% of the total mass):
3.3 SCOPE OF DECLARATION AND SYSTEM BOUNDARIES -Raw materials : Nucleating agent masterbatch
This is a Cradle to gate with options, modules C1-C4 and module CDo nstLCrA.uc tTiheo n lpirofece sscy cslteage (A4-A5)
stages included are as shown below:
(X = module included, ND = module not declared) This stage consists the transport of the product from production plant to the construction
site.
1A A2 A3 A4 A5 B1 B2 B3 B4 B5 B6 B7 C1 C2 C3 C4 D
X X X X X ND ND ND ND ND ND ND X X X X X It also includes the loss of material during construction. The additional needed production,
transport and end-of-life of the lost material during construction is included.
The end-of-life of packaging material up to the end-of-waste state or disposal of final
The modules of the EN15804 contain the following:
residues is also included.
Module 1A = Raw material supply Module B5 = Refurbishment
End of life stage (C1-C4)
Module A2 = Transport Module B6 = Operational energy use
Module A3 = Manufacturing Module B7 = Operational water use
When the end of the life stage of the building is reached, the de-construction/demolition
Module A4 = Transport Module C1 = De-construction / Demolition
begins. This EPD includes de-construction/demolition (C1), the necessary transport (C2)
Module A5 = Construction - from the demolition site to the sorting location and distance to final disposal. The end of
Module C2 = Transport life stage includes the final disposal to landfill (C4), incineration (C3) and needed recycling
Installation process
processes up to the end-of-waste point (C3). Loads and benefits of recycling, re-use and
Module B1 = Use Module C3 = Waste Processing exported energy are part of module D.
ACETex® PP | ReTHiNK-58058 7 / 25
Environmental Product Declaration
3 Calculation rules
The prescribed waste scenarios from the NMD Determination method v1.0 have been used A scaling method was used to calculate the LCA results for the different ACETex® PP
for the various materials in the product. products. The scaling was done on the basis of mass per square meter. As a result of
scaling there are results for both the fixed and the scalable part of the scaling function.
The fixed part means that this number is the same for each product in the product group
Benefits and Loads beyond the system boundary (Module D) and the scalable part is the part that depends on the mass per unit area of the product. In
order to calculate the correct number of each environmental impact category for each of
the products in the product group, the following calculation should be done:
This stage contains the potential loads and benefits of recycling and re-use of raw
materials/products. The loads contain the needed recycling processes from end-of-waste- [number fixed part]+([specific mass]*[number scalable part])
point up to the point-of-equivalence of the substituted primary raw material and a load for
secondary material that will be lost at the end-of-life stage. The inputs slip agent masterbatch, thermoplastic elastomer and cardboard tube were not
having a linear dependance on the specific mass, thus the higher amount of the product
The loads and benefits of recycling and reuse are included in this module. The benefits are available was always considered for the scaling to be as conservative as possible.
calculated based on the primary content and the primary equivalent.
The inputs PP raw yarn, PP chips and PE chips did not have a linear dependence on the
In addition, the benefits of energy recovery are granted at this stage. The amount of avoid specific mass. As they are the main inputs present in the product, the linear dependence
energy is based on the Lower Heating Values of the materials and the efficiencies of the on the specific mass of the sum of these 3 inputs was calculated instead of considering the
incinerators as mentioned in the NMD Determination method v1.0 or EcoInvent 3.6 (2019). inputs separately.
The linear dependence of the energy consumption on the specific mass has been
3.6 ALLOCATION calculated by taking into account the sum of the production energy and the yarn wisting
energy (which is outsourced).
Allocation is based on physical characteristics (mass). The production data was calculated
according to the annual quantity by mass. The raw materials and energy were calculated For C1 the method and amount of the generic data set 'Polyester weefsel' from chapter
according to this allocation key. 22.46 Grondwapening en grondscheiding of the DuboCalc programme (database version
NMD 1.8 - 5.01.14052018) was used. In this generic data set, 0.0013h work per m² of
geotextile was assumed.
3.7 DATA COLLECTION & REFERENCE TIME PERIOD
All process-specific data was collected for the operating year 2021. 3.9 DATA QUALITY
All process-specific data was collected for the 2021 operating year and is therefore up-to-
3.8 ESTIMATES AND ASSUMPTIONS date. The data is based on the annual average. In order to ensure comparability of the
results, only consistent background data of the Ecoinvent database V3.6 was used in the
Almost all datasets chosen for the LCA refer to the RoW as the geographic reference as no LCA (e.g., records on energy, transportation, and supplies), which refers to reference year
national specific environmental profiles were available. 2019. The database is regularly reviewed and thus complies with the requirements of EN
15804 (background data not older than 10 years). All consistent datasets contained in the
Gold-Joint delivers its product to different countries, so the calculation of transport to Ecoinvent database are documented and can be viewed in the online Ecoinvent
construction site (A4) was done by taking the average distance, weighted by the documentation. The primary data were provided by Gold-Joint. The life cycle was modelled
proportion of product shipped to each country. For module A4, a data set for a non- with the R<THiNK EPD App.
specific truck and a transoceanic ship was used.
The following input have been placed under cut-off criteria (<1% of the total mass): 3.10 GUARANTEES OF ORIGIN
-Raw materials : Nucleating agent masterbatch
In this EPD, the local based approach was considered for the LCA, therefore no guaranties
of origin (GO) are needed.
ACETex® PP | ReTHiNK-58058 8 / 25
Environmental Product Declaration
3 Calculation rules
3.12 SCALING
Parameter Value
Scaling type Linear
Description dimension mass
Dimension 0.000
Scalable dimension 1.000
Unit dimension kg/m²
ACETex® PP | ReTHiNK-58058 9 / 25
Environmental Product Declaration
4 Scenarios and additional technical information
4.1 TRANSPORT TO CONSTRUCTION SITE (A4)
For the transport from production place to assembly/user, the following scenario is
assumed for module A4 of this EPD.
Value and unit
Vehicle type used for transport Transoceanic ship / Lorry unspecified
Fuel type and consumption of vehicle
Distance 1705 km
Capacity utilisation (including empty returns)
Bulk density of transported products
Volume capacity utilisation factor
4.2 ASSEMBLY (A5)
The following information describes the scenarios for flows entering the system and flows
leaving the system at module A5.
FLOWS ENTERING THE SYSTEM
There are no significant environment impacts as a result of materials or energy used in the
construction stage (A5).
FLOWS LEAVING THE SYSTEM
The following output flows leaving the system at module A5 are assumed.
Description Value Unit
Output materials as result of loss during construction 5 %
Output materials as result of waste processing of materials used for installation/assembly at the building site 0.000 kg
Output materials as result of waste processing of used packaging 0.086 kg
4.3 DE-CONSTRUCTION, DEMOLITION (C1)
The following information describes the scenario for demolition at end of life.
Description Amount Unit
Hydraulic excavator (average) [NMD] 0.001 hr
ACETex® PP | ReTHiNK-58058 10 / 25
Environmental Product Declaration
4 Scenarios and additional technical information
4.4 TRANSPORT END-OF-LIFE (C2)
The following distances and transport conveyance are assumed for transportation during
end of life for the different types of waste processing.
Waste Scenario Transport conveyance Not removed (stays in Landfill Incineration Recycling Re-use
work) [km] [km] [km] [km] [km]
PE/PP soil reinforcement (geotextile and Lorry (Truck), unspecified (default) | market
0 100 150 50 0
geogrid 54) group for (GLO)
The transport conveyance(s) used in the scenario(s) for transport during end of life has the
following characteristics.
Value and unit
Vehicle type used for transport Lorry (Truck), unspecified (default) | market group for (GLO)
Fuel type and consumption of vehicle not available
Capacity utilisation (including empty returns) 50 % (loaded up and return empty)
Bulk density of transported products inapplicable
Volume capacity utilisation factor 1
4.5 END OF LIFE (C3, C4)
The scenario(s) assumed for end of life of the product are given in the following tables.
First the assumed percentages per type of waste processing are displayed, followed by the
assumed amounts.
Waste Scenario Region Not removed (stays in work) [%] Landfill [%] Incineration [%] Recycling [%] Re-use [%]
PE/PP soil reinforcement (geotextile and geogrid 54) NL 25 0 70 5 0
Waste Scenario Not removed (stays in work) [kg] Landfill [kg] Incineration [kg] Recycling [kg] Re-use [kg]
PE/PP soil reinforcement (geotextile and geogrid 54) 0.348 0.000 0.976 0.070 0.000
Total 0.348 0.000 0.976 0.070 0.000
ACETex® PP | ReTHiNK-58058 11 / 25
Environmental Product Declaration
4 Scenarios and additional technical information
4.6 BENEFITS AND LOADS BEYOND THE SYSTEM BOUNDARY (D)
The presented Benefits and loads beyond the system boundary in this EPD are based on
the following calculated Net output flows in kilograms and Energy recovery displayed in
MJ Lower Heating Value.
Waste Scenario Net output flow [kg] Energy recovery [MJ]
PE/PP soil reinforcement (geotextile and geogrid 54) 0.067 32.155
Total 0.067 32.155
ACETex® PP | ReTHiNK-58058 12 / 25
Environmental Product Declaration
5 Results
For the impact assessment, the characterization factors of the LCIA method EN 15804 +A2
Method v1.0 are used. Long-term emissions (>100 years) are not considered in the impact
assessment. The results of the impact assessment are only relative statements that do not
make any statements about end-points of the impact categories, exceedance of threshold
values, safety margins or risks. The following tables show the results of the indicators of the
impact assessment, of the use of resources as well as of waste and other output flows.
ACETex® PP | ReTHiNK-58058 13 / 25
Environmental Product Declaration
5 Results
5.1 ENVIRONMENTAL IMPACT INDICATORS PER SQUARE METER (FIXED PART)
CORE ENVIRONMENTAL IMPACT INDICATORS EN15804+A2
Abbreviation Unit A1 A2 A3 A4 A5 C1 C2 C3 C4 D
AP mol H+ eqv. -1.99E-4 -4.01E-6 2.26E-4 8.67E-6 1.67E-5 7.12E-4 -2.33E-6 -1.30E-5 -3.54E-7 6.59E-5
GWP-total kg CO2 eqv. -5.00E-2 -6.92E-4 4.80E-2 7.40E-4 7.21E-2 6.81E-2 -4.02E-4 -2.87E-2 -5.68E-4 7.91E-2
GWP-b kg CO2 eqv. -4.17E-4 -3.19E-7 -9.42E-4 4.58E-7 7.54E-2 1.89E-5 -1.86E-7 -4.16E-6 -4.37E-7 2.96E-5
GWP-f kg CO2 eqv. -4.95E-2 -6.91E-4 4.87E-2 7.39E-4 -3.30E-3 6.81E-2 -4.02E-4 -2.87E-2 -5.67E-4 7.91E-2
GWP-luluc kg CO2 eqv. -2.43E-5 -2.53E-7 2.43E-4 3.06E-7 1.14E-5 5.37E-6 -1.47E-7 -2.33E-6 -2.00E-8 -1.58E-5
EP-m kg N eqv. -3.63E-5 -1.41E-6 6.11E-5 2.15E-6 7.27E-6 3.14E-4 -8.21E-7 -3.54E-6 -2.14E-7 1.87E-5
EP-fw kg P eqv. -1.30E-6 -6.98E-9 2.19E-6 8.71E-9 7.14E-8 2.48E-7 -4.05E-9 -8.66E-8 -7.27E-10 -3.68E-9
EP-T mol N eqv. -4.12E-4 -1.56E-5 5.99E-4 2.40E-5 7.44E-5 3.45E-3 -9.05E-6 -3.94E-5 -1.30E-6 2.06E-4
kg CFC 11
ODP 6.07E-9 -1.53E-10 5.44E-9 1.57E-10 8.08E-10 1.47E-8 -8.87E-11 -8.79E-10 -1.25E-11 1.00E-8
eqv.
kg NMVOC
POCP -1.86E-4 -4.45E-6 1.27E-4 6.57E-6 1.72E-5 9.49E-4 -2.59E-6 -1.06E-5 -4.98E-7 6.74E-5
eqv.
ADP-f MJ -1.93E+0 -1.04E-2 5.15E-1 1.09E-2 -5.36E-2 9.37E-1 -6.06E-3 -2.24E-2 -9.60E-4 1.36E+0
ADP-mm kg Sb-eqv. -2.61E-7 -1.75E-8 3.63E-7 1.29E-8 7.73E-8 1.04E-7 -1.02E-8 -3.68E-8 -4.34E-10 2.23E-8
m3 world
WDP -7.41E-3 -3.73E-5 1.17E-2 4.79E-5 1.70E-4 1.26E-3 -2.17E-5 -1.47E-3 -4.11E-5 6.99E-3
eqv.
AP=Acidification (AP) | GWP-total=Global warming potential (GWP-total) | GWP-b=Global warming potential - Biogenic (GWP-b) | GWP-f=Global warming potential - Fossil (GWP-f) | GWP-
luluc=Global warming potential - Land use and land use change (GWP-luluc) | EP-m=Eutrophication marine (EP-m) | EP-fw=Eutrophication, freshwater (EP-fw) | EP-T=Eutrophication,
terrestrial (EP-T) | ODP=Ozone depletion (ODP) | POCP=Photochemical ozone formation - human health (POCP) | ADP-f=Resource use, fossils (ADP-f) | ADP-mm=Resource use, minerals and
metals (ADP-mm) | WDP=Water use (WDP)
ACETex® PP | ReTHiNK-58058 14 / 25
Environmental Product Declaration
5 Results
ADDITIONAL ENVIRONMENTAL IMPACT INDICATORS EN15084+A2
Abbreviation Unit A1 A2 A3 A4 A5 C1 C2 C3 C4 D
ETP-fw CTUe -2.25E-1 -9.30E-3 3.64E+0 9.01E-3 1.76E-1 5.65E-1 -5.40E-3 -3.61E-1 -1.02E-3 7.55E-2
disease
PM -8.41E-10 -6.22E-11 2.77E-9 5.23E-11 3.51E-10 1.89E-8 -3.62E-11 -1.05E-10 -6.67E-12 1.79E-10
incidence
HTP-c CTUh -9.45E-12 -3.02E-13 3.79E-11 2.95E-13 6.17E-12 1.97E-11 -1.75E-13 -5.50E-12 -2.68E-14 4.69E-12
HTP-nc CTUh -3.53E-11 -1.02E-11 5.86E-10 9.13E-12 6.61E-11 4.85E-10 -5.91E-12 -1.14E-10 -6.65E-13 6.28E-11
IR kBq U235 eqv. 1.03E-3 -4.37E-5 1.82E-3 4.66E-5 2.60E-4 4.02E-3 -2.54E-5 -9.17E-5 -3.76E-6 4.12E-4
SQP Pt 3.25E-2 -9.04E-3 1.45E+0 6.95E-3 8.56E-2 1.20E-1 -5.26E-3 -8.25E-3 -2.27E-3 -2.29E+0
ETP-fw=Ecotoxicity, freshwater (ETP-fw) | PM=Particulate Matter (PM) | HTP-c=Human toxicity, cancer (HTP-c) | HTP-nc=Human toxicity, non-cancer (HTP-nc) | IR=Ionising radiation, human
health (IR) | SQP=Land use (SQP)
CLASSIFICATION OF DISCLAIMERS TO THE DECLARATION OF CORE AND ADDITIONAL ENVIRONMENTAL IMPACT INDICATORS
ILCD classification Indicator Disclaimer
Global warming potential (GWP) None
ILCD type / level 1 Depletion potential of the stratospheric ozone layer (ODP) None
Potential incidence of disease due to PM emissions (PM) None
AAcidification potential, Accumulated Exceedance (AP) None
Eutrophication potential, Fraction of nutrients reaching freshwater end compartment
None
(EP-freshwater)
Eutrophication potential, Fraction of nutrients reaching marine end compartment
ILCD type / level 2 None
(EP-marine)
Eutrophication potential, Accumulated Exceedance (EP-terrestrial) None
Formation potential of tropospheric ozone (POCP) None
Potential Human exposure efficiency relative to U235 (IRP) 1
Abiotic depletion potential for non-fossil resources (ADP-minerals&metals) 2
ILCD type / level 3
Abiotic depletion potential for fossil resources (ADP-fossil) 2
Water (user) deprivation potential, deprivation-weighted water consumption (WDP) 2
Potential Comparative Toxic Unit for ecosystems (ETP-fw) 2
ACETex® PP | ReTHiNK-58058 15 / 25
Environmental Product Declaration
5 Results
ILCD classification Indicator Disclaimer
Potential Comparative Toxic Unit for humans (HTP-c) 2
Potential Comparative Toxic Unit for humans (HTP-nc) 2
Potential Soil quality index (SQP) 2
Disclaimer 1 – This impact category deals mainly with the eventual impact of low dose ionizing radiation on human health of the nuclear fuel cycle. It does not consider effects due to possible
nuclear accidents, occupational exposure nor due to radioactive waste disposal in underground facilities. Potential ionizing radiation from the soil, from radon and from some construction
materials is also not measured by this indicator.
Disclaimer 2 – The results of this environmental impact indicator shall be used with care as the uncertainties on these results are high or as there is limited experienced with the indicator.
5.2 ENVIRONMENTAL IMPACT INDICATORS PER SQUARE METER (SCALABLE PART)
CORE ENVIRONMENTAL IMPACT INDICATORS EN15804+A2
Abbreviation Unit A1 A2 A3 A4 A5 C1 C2 C3 C4 D
AP mol H+ eqv. 1.40E-2 2.28E-4 2.88E-3 8.24E-4 1.02E-3 0.00E+0 1.13E-4 1.14E-3 3.11E-5 -1.80E-3
GWP-total kg CO2 eqv. 3.39E+0 3.94E-2 8.61E-1 7.03E-2 4.65E-1 0.00E+0 1.95E-2 2.53E+0 4.99E-2 -1.71E+0
GWP-b kg CO2 eqv. 8.43E-3 1.82E-5 2.45E-4 4.35E-5 4.81E-4 0.00E+0 9.01E-6 3.66E-4 3.84E-5 -1.17E-3
GWP-f kg CO2 eqv. 3.38E+0 3.93E-2 8.60E-1 7.02E-2 4.64E-1 0.00E+0 1.95E-2 2.53E+0 4.99E-2 -1.71E+0
GWP-luluc kg CO2 eqv. 1.85E-3 1.44E-5 2.92E-4 2.91E-5 1.29E-4 0.00E+0 7.15E-6 2.05E-4 1.76E-6 -8.89E-5
EP-m kg N eqv. 2.47E-3 8.04E-5 4.75E-4 2.05E-4 1.98E-4 0.00E+0 3.99E-5 3.11E-4 1.89E-5 -4.73E-4
EP-fw kg P eqv. 8.27E-5 3.97E-7 1.86E-5 8.28E-7 5.86E-6 0.00E+0 1.97E-7 7.62E-6 6.40E-8 -4.15E-6
EP-T mol N eqv. 2.75E-2 8.86E-4 5.31E-3 2.28E-3 2.20E-3 0.00E+0 4.40E-4 3.47E-3 1.14E-4 -5.21E-3
kg CFC 11
ODP 9.77E-8 8.68E-9 1.33E-8 1.50E-8 1.56E-8 0.00E+0 4.31E-9 7.73E-8 1.10E-9 -2.07E-7
eqv.
kg NMVOC
POCP 1.10E-2 2.53E-4 2.11E-3 6.24E-4 8.10E-4 0.00E+0 1.26E-4 9.32E-4 4.38E-5 -1.88E-3
eqv.
AP=Acidification (AP) | GWP-total=Global warming potential (GWP-total) | GWP-b=Global warming potential - Biogenic (GWP-b) | GWP-f=Global warming potential - Fossil (GWP-f) | GWP-
luluc=Global warming potential - Land use and land use change (GWP-luluc) | EP-m=Eutrophication marine (EP-m) | EP-fw=Eutrophication, freshwater (EP-fw) | EP-T=Eutrophication,
terrestrial (EP-T) | ODP=Ozone depletion (ODP) | POCP=Photochemical ozone formation - human health (POCP) | ADP-f=Resource use, fossils (ADP-f) | ADP-mm=Resource use, minerals and
metals (ADP-mm) | WDP=Water use (WDP)
ACETex® PP | ReTHiNK-58058 16 / 25
Environmental Product Declaration
5 Results
Abbreviation Unit A1 A2 A3 A4 A5 C1 C2 C3 C4 D
ADP-f MJ 1.03E+2 5.93E-1 1.47E+1 1.04E+0 6.36E+0 0.00E+0 2.94E-1 1.97E+0 8.45E-2 -3.12E+1
ADP-mm kg Sb-eqv. 3.45E-5 9.97E-7 6.30E-6 1.23E-6 2.51E-6 0.00E+0 4.95E-7 3.24E-6 3.82E-8 -1.71E-6
m3 world
WDP 1.26E+0 2.12E-3 2.06E-1 4.56E-3 8.71E-2 0.00E+0 1.05E-3 1.29E-1 3.62E-3 -2.30E-1
eqv.
AP=Acidification (AP) | GWP-total=Global warming potential (GWP-total) | GWP-b=Global warming potential - Biogenic (GWP-b) | GWP-f=Global warming potential - Fossil (GWP-f) | GWP-
luluc=Global warming potential - Land use and land use change (GWP-luluc) | EP-m=Eutrophication marine (EP-m) | EP-fw=Eutrophication, freshwater (EP-fw) | EP-T=Eutrophication,
terrestrial (EP-T) | ODP=Ozone depletion (ODP) | POCP=Photochemical ozone formation - human health (POCP) | ADP-f=Resource use, fossils (ADP-f) | ADP-mm=Resource use, minerals and
metals (ADP-mm) | WDP=Water use (WDP)
ADDITIONAL ENVIRONMENTAL IMPACT INDICATORS EN15084+A2
Abbreviation Unit A1 A2 A3 A4 A5 C1 C2 C3 C4 D
ETP-fw CTUe 3.96E+1 5.29E-1 1.26E+1 8.56E-1 5.63E+0 0.00E+0 2.63E-1 3.18E+1 8.98E-2 -2.33E+0
disease
PM 1.12E-7 3.54E-9 2.00E-8 4.97E-9 8.11E-9 0.00E+0 1.76E-9 9.23E-9 5.87E-10 -7.95E-9
incidence
HTP-c CTUh 8.46E-10 1.72E-11 2.25E-10 2.80E-11 1.02E-10 0.00E+0 8.52E-12 4.84E-10 2.36E-12 -1.37E-10
HTP-nc CTUh 2.51E-8 5.79E-10 6.45E-9 8.68E-10 2.61E-9 0.00E+0 2.87E-10 1.00E-8 5.85E-11 -2.28E-9
IR kBq U235 eqv. 6.06E-2 2.49E-3 1.71E-2 4.43E-3 5.17E-3 0.00E+0 1.23E-3 8.06E-3 3.30E-4 -1.18E-2
SQP Pt 4.53E+0 5.15E-1 1.09E+0 6.61E-1 4.45E-1 0.00E+0 2.55E-1 7.25E-1 2.00E-1 -5.43E-1
ETP-fw=Ecotoxicity, freshwater (ETP-fw) | PM=Particulate Matter (PM) | HTP-c=Human toxicity, cancer (HTP-c) | HTP-nc=Human toxicity, non-cancer (HTP-nc) | IR=Ionising radiation, human
health (IR) | SQP=Land use (SQP)
CLASSIFICATION OF DISCLAIMERS TO THE DECLARATION OF CORE AND ADDITIONAL ENVIRONMENTAL IMPACT INDICATORS
ILCD classification Indicator Disclaimer
Global warming potential (GWP) None
ILCD type / level 1 Depletion potential of the stratospheric ozone layer (ODP) None
Potential incidence of disease due to PM emissions (PM) None
AAcidification potential, Accumulated Exceedance (AP) None
ILCD type / level 2
None
ACETex® PP | ReTHiNK-58058 17 / 25
Environmental Product Declaration
5 Results
ILCD classification Indicator Disclaimer
Eutrophication potential, Fraction of nutrients reaching freshwater end compartment
(EP-freshwater)
Eutrophication potential, Fraction of nutrients reaching marine end compartment
None
(EP-marine)
Eutrophication potential, Accumulated Exceedance (EP-terrestrial) None
Formation potential of tropospheric ozone (POCP) None
Potential Human exposure efficiency relative to U235 (IRP) 1
Abiotic depletion potential for non-fossil resources (ADP-minerals&metals) 2
Abiotic depletion potential for fossil resources (ADP-fossil) 2
Water (user) deprivation potential, deprivation-weighted water consumption (WDP) 2
ILCD type / level 3 Potential Comparative Toxic Unit for ecosystems (ETP-fw) 2
Potential Comparative Toxic Unit for humans (HTP-c) 2
Potential Comparative Toxic Unit for humans (HTP-nc) 2
Potential Soil quality index (SQP) 2
Disclaimer 1 – This impact category deals mainly with the eventual impact of low dose ionizing radiation on human health of the nuclear fuel cycle. It does not consider effects due to possible
nuclear accidents, occupational exposure nor due to radioactive waste disposal in underground facilities. Potential ionizing radiation from the soil, from radon and from some construction
materials is also not measured by this indicator.
Disclaimer 2 – The results of this environmental impact indicator shall be used with care as the uncertainties on these results are high or as there is limited experienced with the indicator.
ACETex® PP | ReTHiNK-58058 18 / 25
Environmental Product Declaration
5 Results
5.3 ENVIRONMENTAL IMPACT INDICATORS PER SQUARE METER (FIXED PART)
PARAMETERS DESCRIBING RESOURCE USE
Abbreviation Unit A1 A2 A3 A4 A5 C1 C2 C3 C4 D
PERE MJ -1.57E-2 -1.31E-4 2.78E-1 1.63E-4 1.38E-2 5.07E-3 -7.59E-5 -2.27E-3 -1.70E-5 -3.94E-1
PERM MJ 0.00E+0 0.00E+0 0.00E+0 0.00E+0 0.00E+0 0.00E+0 0.00E+0 0.00E+0 0.00E+0 0.00E+0
PERT MJ -1.57E-2 -1.31E-4 2.78E-1 1.63E-4 1.38E-2 5.07E-3 -7.59E-5 -2.27E-3 -1.70E-5 -3.94E-1
PENRE MJ -1.12E+0 -1.11E-2 1.06E-1 1.16E-2 -3.24E-2 9.95E-1 -6.43E-3 -2.38E-2 -1.02E-3 1.47E+0
PENRM MJ -9.46E-1 0.00E+0 4.53E-1 0.00E+0 -2.55E-2 0.00E+0 0.00E+0 0.00E+0 0.00E+0 3.74E-2
PENRT MJ -2.07E+0 -1.11E-2 5.59E-1 1.16E-2 -5.78E-2 9.95E-1 -6.43E-3 -2.38E-2 -1.02E-3 1.50E+0
SM Kg 0.00E+0 0.00E+0 0.00E+0 0.00E+0 0.00E+0 0.00E+0 0.00E+0 0.00E+0 0.00E+0 0.00E+0
RSF MJ 0.00E+0 0.00E+0 0.00E+0 0.00E+0 0.00E+0 0.00E+0 0.00E+0 0.00E+0 0.00E+0 0.00E+0
NRSF MJ 0.00E+0 0.00E+0 0.00E+0 0.00E+0 0.00E+0 0.00E+0 0.00E+0 0.00E+0 0.00E+0 0.00E+0
FW M3 -1.66E-4 -1.27E-6 3.75E-4 1.57E-6 1.62E-5 4.83E-5 -7.38E-7 -4.31E-5 -1.00E-6 9.34E-5
PERE=renewable primary energy ex. raw materials | PERM=renewable primary energy used as raw materials | PERT=renewable primary energy total | PENRE=non-renewable primary energy
ex. raw materials | PENRM=non-renewable primary energy used as raw materials | PENRT=non-renewable primary energy total | SM=use of secondary material | RSF=use of renewable
secondary fuels | NRSF=use of non-renewable secondary fuels | FW=use of net fresh water
OTHER ENVIRONMENTAL INFORMATION DESCRIBING WASTE CATEGORIES
Abbreviation Unit A1 A2 A3 A4 A5 C1 C2 C3 C4 D
HWD Kg 1.28E-7 -2.64E-8 8.83E-7 2.17E-8 1.18E-7 2.55E-6 -1.54E-8 -4.27E-8 -1.46E-9 1.61E-6
NHWD Kg -2.63E-3 -6.62E-4 6.76E-3 4.75E-4 7.73E-4 1.11E-3 -3.84E-4 -5.52E-4 -3.83E-3 2.09E-4
RWD Kg 2.35E-6 -6.85E-8 2.00E-6 7.16E-8 3.92E-7 6.51E-6 -3.98E-8 -8.05E-8 -5.71E-9 5.85E-7
HWD=hazardous waste disposed | NHWD=non hazardous waste disposed | RWD=radioactive waste disposed
ACETex® PP | ReTHiNK-58058 19 / 25
Environmental Product Declaration
5 Results
ENVIRONMENTAL INFORMATION DESCRIBING OUTPUT FLOWS
Abbreviation Unit A1 A2 A3 A4 A5 C1 C2 C3 C4 D
CRU Kg 0.00E+0 0.00E+0 0.00E+0 0.00E+0 0.00E+0 0.00E+0 0.00E+0 0.00E+0 0.00E+0 0.00E+0
MFR Kg 0.00E+0 0.00E+0 -3.76E-4 0.00E+0 3.45E-2 0.00E+0 0.00E+0 -7.65E-4 0.00E+0 0.00E+0
MER Kg 0.00E+0 0.00E+0 0.00E+0 0.00E+0 0.00E+0 0.00E+0 0.00E+0 0.00E+0 0.00E+0 0.00E+0
EET MJ 0.00E+0 0.00E+0 -7.66E-2 0.00E+0 0.00E+0 0.00E+0 0.00E+0 0.00E+0 0.00E+0 -5.81E-1
EEE MJ 0.00E+0 0.00E+0 -4.45E-2 0.00E+0 0.00E+0 0.00E+0 0.00E+0 0.00E+0 0.00E+0 -3.37E-1
CRU=Components for re-use | MFR=Materials for recycling | MER=Materials for energy recovery | EET=Exported Energy Thermic | EEE=Exported Energy Electric
5.4 ENVIRONMENTAL IMPACT INDICATORS PER SQUARE METER (SCALABLE PART)
PARAMETERS DESCRIBING RESOURCE USE
Abbreviation Unit A1 A2 A3 A4 A5 C1 C2 C3 C4 D
PERE MJ 1.66E+0 7.43E-3 3.60E-1 1.55E-2 1.22E-1 0.00E+0 3.69E-3 1.99E-1 1.49E-3 -1.42E-1
PERM MJ 0.00E+0 0.00E+0 0.00E+0 0.00E+0 0.00E+0 0.00E+0 0.00E+0 0.00E+0 0.00E+0 0.00E+0
PERT MJ 1.66E+0 7.43E-3 3.60E-1 1.55E-2 1.22E-1 0.00E+0 3.69E-3 1.99E-1 1.49E-3 -1.42E-1
PENRE MJ 6.17E+1 6.30E-1 8.37E+0 1.10E+0 4.02E+0 0.00E+0 3.13E-1 2.09E+0 8.98E-2 -3.14E+1
PENRM MJ 4.84E+1 0.00E+0 7.25E+0 0.00E+0 2.80E+0 0.00E+0 0.00E+0 0.00E+0 0.00E+0 -3.08E+0
PENRT MJ 1.10E+2 6.30E-1 1.56E+1 1.10E+0 6.82E+0 0.00E+0 3.13E-1 2.09E+0 8.98E-2 -3.45E+1
SM Kg 0.00E+0 0.00E+0 0.00E+0 0.00E+0 0.00E+0 0.00E+0 0.00E+0 0.00E+0 0.00E+0 0.00E+0
RSF MJ 0.00E+0 0.00E+0 0.00E+0 0.00E+0 0.00E+0 0.00E+0 0.00E+0 0.00E+0 0.00E+0 0.00E+0
NRSF MJ 0.00E+0 0.00E+0 0.00E+0 0.00E+0 0.00E+0 0.00E+0 0.00E+0 0.00E+0 0.00E+0 0.00E+0
FW M3 3.15E-2 7.23E-5 5.62E-3 1.49E-4 2.24E-3 0.00E+0 3.59E-5 3.79E-3 8.81E-5 -3.27E-3
PERE=renewable primary energy ex. raw materials | PERM=renewable primary energy used as raw materials | PERT=renewable primary energy total | PENRE=non-renewable primary energy
ex. raw materials | PENRM=non-renewable primary energy used as raw materials | PENRT=non-renewable primary energy total | SM=use of secondary material | RSF=use of renewable
secondary fuels | NRSF=use of non-renewable secondary fuels | FW=use of net fresh water
ACETex® PP | ReTHiNK-58058 20 / 25
Environmental Product Declaration
5 Results
OTHER ENVIRONMENTAL INFORMATION DESCRIBING WASTE CATEGORIES
Abbreviation Unit A1 A2 A3 A4 A5 C1 C2 C3 C4 D
HWD Kg 1.53E-5 1.50E-6 5.11E-7 2.06E-6 1.61E-6 0.00E+0 7.46E-7 3.75E-6 1.28E-7 -3.37E-5
NHWD Kg 1.95E-1 3.76E-2 6.86E-2 4.51E-2 4.50E-2 0.00E+0 1.87E-2 4.86E-2 3.37E-1 -1.51E-2
RWD Kg 5.29E-5 3.90E-6 1.55E-5 6.81E-6 4.91E-6 0.00E+0 1.93E-6 7.08E-6 5.02E-7 -1.55E-5
HWD=hazardous waste disposed | NHWD=non hazardous waste disposed | RWD=radioactive waste disposed
ENVIRONMENTAL INFORMATION DESCRIBING OUTPUT FLOWS
Abbreviation Unit A1 A2 A3 A4 A5 C1 C2 C3 C4 D
CRU Kg 0.00E+0 0.00E+0 0.00E+0 0.00E+0 0.00E+0 0.00E+0 0.00E+0 0.00E+0 0.00E+0 0.00E+0
MFR Kg 0.00E+0 0.00E+0 8.22E-3 0.00E+0 6.07E-3 0.00E+0 0.00E+0 6.73E-2 0.00E+0 0.00E+0
MER Kg 0.00E+0 0.00E+0 0.00E+0 0.00E+0 0.00E+0 0.00E+0 0.00E+0 0.00E+0 0.00E+0 0.00E+0
EET MJ 0.00E+0 0.00E+0 1.51E+0 0.00E+0 0.00E+0 0.00E+0 0.00E+0 0.00E+0 0.00E+0 1.16E+1
EEE MJ 0.00E+0 0.00E+0 8.79E-1 0.00E+0 0.00E+0 0.00E+0 0.00E+0 0.00E+0 0.00E+0 6.74E+0
CRU=Components for re-use | MFR=Materials for recycling | MER=Materials for energy recovery | EET=Exported Energy Thermic | EEE=Exported Energy Electric
ACETex® PP | ReTHiNK-58058 21 / 25
Environmental Product Declaration
5 Results
5.5 INFORMATION ON BIOGENIC CARBON CONTENT PER SQUARE METER
BIOGENIC CARBON CONTENT
The following Information describes the biogenic carbon content in (the main parts of) the
product at the factory gate per square meter:
Biogenic carbon content Amount Unit
Biogenic carbon content in the product 0 kg C
Biogenic carbon content in accompanying packaging 0 kg C
ACETex® PP | ReTHiNK-58058 22 / 25
Environmental Product Declaration
6 Interpretation of results
As shown in the figure below, the raw material supply (A1) dominates in most
environmental core indicators, followed by production process (A3). The highest influence
on the Global Warming Potential (GWP-total) have raw material supply (A1) and waste
processing (C3).
ACETex® PP | ReTHiNK-58058 23 / 25
Environmental Product Declaration
7 References
ISO 14040
ISO 14040:2006-10, Environmental management - Life cycle assessment - Principles and
framework; EN ISO 14040:2006
ISO 14044
ISO 14044:2006-10, Environmental management - Life cycle assessment - Requirements
and guidelines; EN ISO 14040:2006
ISO 14025
ISO 14025:2011-10: Environmental labels and declarations — Type III environmental
declarations — Principles and procedures
EN 15804+A2
EN 15804+A2: 2019: Sustainability of construction works — Environmental Product
Declarations — Core rules for the product category of construction products
PCR A: General Program Category Rules for Construction Products from the EPD program
Kiwa-Ecobility Experts, 2022-02-14
PCR B: Product Category Rules (PCR) from the Kiwa-Ecobility Experts (Kiwa-EE) – Specific
Product Category Rules: Geosynthetic products, 2023-07-21
ACETex® PP | ReTHiNK-58058 24 / 25
Environmental Product Declaration
8 Contact information
Publisher Operator Owner of declaration
Kiwa-Ecobility Experts Kiwa-Ecobility Experts Gold-Joint Industry Co., Ltd.
Voltastraße 5 Voltastraße 5 No.33, Jing 3 Rd. Wuqi Dist.
13355 Berlin, DE 13355 Berlin, DE 43541 Taichung City, Taiwan (R.O.C.), TW
E-mail: E-mail: E-mail:
DE.Ecobility.Experts@kiwa.com DE.Ecobility.Experts@kiwa.com marketing@geoace.com
Website: Website: Website:
https://www.kiwa.com/de/en/themes/ecobility-experts/ecobility-https://www.kiwa.com/de/en/themes/ecobility-experts/ecobility-www.geoace.com
experts-epd-program/ experts-epd-program/
Kiwa-Ecobility Experts is
established member of the
ACETex® PP | ReTHiNK-58058 25 / 25
