ENVIRONMENTAL PRODUCT DECLARATION
as per ISO 14025 and EN 15804+A2
Owner of the Declaration Hansgrohe Group
Programme holder Institut Bauen und Umwelt e.V. (IBU)
Publisher Institut Bauen und Umwelt e.V. (IBU)
Declaration number EPD-HAN-20230024-ICC1-EN
Issue date 24.02.2023
Valid to 23.02.2028
Kitchen faucets
Hansgrohe Group
www.ibu-epd.com | https://epd-online.com
Umwelt Produktdeklaration Name des Herstellers – Name des Produkts
1. General Information
Hansgrohe Group Kitchen Faucets
Programme holder Owner of the declaration
IBU – Institut Bauen und Umwelt e.V. Hansgrohe Group
Hegelplatz 1 Auestraße 5 - 9
10117 Berlin 77761 Schiltach
Germany Germany
Declaration number Declared product / declared unit
EPD-HAN-20230024-ICC1-EN One (1) piece of an average kitchen faucet incl.
packaging
This declaration is based on the product Scope:
category rules: This average EPD was determined on the basis of a
Fittings and showers, 07.2014 weighted average of production volume from 2021 and
(PCR checked and approved by the SVR) relates to the plants in Offenburg and Schiltach,
Germany, Shanghai, China and Alpharetta, USA. This
average EPD is valid for the whole product group of
Issue date
chrome plated kitchen faucets. The EPD was formed
24.02.2023
from >85% of the products involved in the sales
quantity.
Valid to
23.02.2028
The owner of the declaration shall be liable for the
underlying information and evidence; the IBU shall not
be liable with respect to manufacturer information, life
cycle assessment data and evidences.
The EPD was created according to the specifications
of EN 15804+A2. In the following, the standard will be
simplified as EN 15804.
Verification
The standard EN 15804 serves as the core PCR
Independent verification of the declaration and data
according to ISO 14025:2011
Dipl. Ing. Hans Peters internally x externally
(chairman of Institut Bauen und Umwelt e.V.)
Dr. Alexander Röder Dr Naeem Adibi
(Managing Director Institut Bauen und Umwelt e.V.)) (Independent verifier)
2. Product
2.1 Product description/Product definition  EN 816:2017: Sanitary tapware – Automatic
Kitchen faucets essentially comprise of a metal shut-off valves PN 10
housing in most cases made of brass, a plastic valve
 EN 817:2008: Sanitary tapware – Mechanical
with ceramic discs and several assembly parts of
mixing valves (PN 10)
various materials. The faucet surface is usually
chrome-plated by means of various galvanic process  EN 200:2008: Sanitary tapware – Single taps
stages. and combination taps for water supply
systems of type 1 and type 2
For the use and application of the products the  ISO 3822: Acoustics – Laboratory tests on
respective national provisions at the place of use
noise emission from appliances and
apply, in Germany for example the building codes of
equipment used in water supply installations
the federal states and the corresponding national
specifications.
2.2 Application
The products comply with the applicable standards and Kitchen faucets are fixtures that mix hot and cold
regulations listed below. water, shut off water, and regulate the amount of
water. They are mechanically operated by handles and
Following standards depending on the operating are used for dish washing, washing of vegetables and
mechanism may apply to taps and roughs to prove fruits, filling pots with water and hand washing in
product safety: kitchens.
2 Environmental Product Declaration Hansgrohe Group – Kitchen Faucets
2.3 Technical Data 2.6 Manufacture
Constructional data
Name Value Unit
Maximum load temperature permanent
65 °C
operation
Maximum load temperature temporary
90 °C
operation
Dependi
ng on
Flow rate (indications for pressure the
m3/h
range of 1-3 bar) product
0,09 to
1,2
Sound emissions < 30 dB
Performance data of the product with respect to its
characteristics in accordance with the relevant
technical provision (no CE-marking). No. 1: The sand core for the base body is made.
No. 2: The body of the faucet is cast from brass using
2.4 Delivery status the sand core.
The Kitchen Faucets are delivered singularly No. 3: After casting, the brass body is grinded and
packaged. The packaging is customized to the size of polished.
the product and supplies. Customers can order single No. 4: To protect the product and make it durable, the
products or multiple products with outer packaging. body is galvanized with chrome.
The products with the smallest and the largest volume No. 5: Meanwhile, the individual parts of the cartridge
have dimensions between 280x65x370 mm and are assembled.
325x118x558 mm. No. 6: The product parts (chrome plated brass body,
cartridge, chrome-plated outlet bow with soldered
2.5 Base materials/Ancillary materials sleeve, chrome plated handle and others) are
assembled.
The material composition (incl. packaging) of an No. 7: The preassembled product is packed together
average kitchen faucet is as follows: with the remaining components (like fastening parts).
Name Value Unit Any production waste generated is disposed
Lead 3.0 % accordingly. In individual cases, the production may
Stainless Steel 1.9 % differ slightly from the procedure (for example, if the
Brass 44.8 % brass body is purchased and not manufactured in-
Steel 0.1 % house).
Zinc 17.0 %
2.7 Environment and health during
Polyphenylensulfide 3.2 %
manufacturing
Polyethylene 5.8 %
Hansgrohe SE tries to keep the impact on people and
Other Plastics 4.0 %
the environment as low as possible when
Other Materials 1.0 %
manufacturing its products.
Cardboard, Paper 19.0 %
Hazards at workplaces are regularly assessed and
reduced to a minimum.
The parts which are made of brass contain between
For example, in basic production, sawing or grinding
0.2 and 1.4% lead.
work is mainly carried out by robots, and in
This product contains substances listed in the
electroplating, chemicals are dosed automatically via
candidate list (date: 17.12.2021) exceeding 0.1
appropriate pump stations.
percentage by mass: Lead (CAS number 7439-92-1)
Emissions that are hazardous to health are extracted
as a component of the brass alloy has been on the
directly at the source and cleaned by filter systems.
candidate list of the Reach Regulation (Regulation
Workplace and emission limits are regularly monitored
(EC) No. 1907/2006) since 27.06.2018.
and are far below the prescribed limits.
To reduce environmental impact, water and production
This product/article/at least one partial article contains
waste are recycled wherever possible.
other CMR substances in categories 1A or 1B which
In addition, all production sites are certified according
are not on the candidate list, exceeding 0.1 percentage
to the DIN EN
by mass: no.
ISO standards 14001 (environment), 50001 (energy), 4
5001 (occupational health and safety)
Biocide products were added to this construction
and 9001 (quality). Continuous improvement of
product or it has been treated with biocide products
environmental and occupational safety performance is
(this then concerns a treated product as defined by the
thus guaranteed.
(EU) Ordinance on Biocide Products No.
528/2012): no.
2.8 Product processing/Installation
The fitting is screwed to the kitchen sink or countertop
(tools: wrench or screwdriver).
The supply hoses are connected to the angle valve.
3 Environmental Product Declaration Hansgrohe Group – Kitchen Faucets
The handle is removed to adjust the temperature The products are not classified as building materials
setting of the cartridge and to adjust the anti-scald (building products) and are not subject to DIN 4102
protection (tools: hexagonal offset screwdriver and and EN 13501-1.
pliers).
The handle is then reattached (tool: hexagonal offset Fire protection
screwdriver). Name Value
Building material class -
2.9 Packaging Burning droplets -
For product protection the kitchen faucets are Smoke gas development -
individually packed in a cardboard box, which consists
of approximately 80% recycled material. The Water
cardboard is always printed with lead-free ink and in If a room in which the products offered by Hansgrohe
some cases additionally coated with clear topcoat. The are installed is flooded with water, the electronic
inlay of the packaging consists of folded cardboard, faucets may be destroyed. All other products are not
fiber form or plastic bags, depending on the product. affected in their function.
The packaging can be fully recycled. There will be no environmental impact.
All packaged products fit on a reusable euro pallet.
Mechanical destruction
If the surface of the coating is destroyed by a
2.10 Condition of use mechanical stress, there is a possibility of corrosion.
To protect the kitchen faucets and make them durable, In the event of mechanical damage, the products may
the body and handle are made of chrome-plated metal. need to be replaced due to possible sharp cut edges.
Nevertheless, there are no unhealthy contaminants in
the water and drinking water quality is guaranteed. To 2.14 Re-use phase
ensure the longevity of the product, it should be used The basin faucets are not taken back by the
daily and cleaned regularly. manufacturer for the purpose of reuse. Users can
disassemble the products repeatedly within the
2.11 Environment and health during use reference utilization period and reuse it elsewhere.
Our products do not emission any contaminants or
substances that are harmful to the environment or 2.15 Disposal
health during the use phase. The waste code of the product is AVV 20 03 01.
Disassembly of the products consists of the same
2.12 Reference service life steps as assembly, in reverse order.
The quality and durability of our kitchen faucets is All metal components can be recycled (as scrap).
designed for a product life of about ten years. Which All plastic components have a high calorific value and
on average is approximately the duration of use by the can be sent for thermal recycling.
consumers. In countries where no thermal recycling or substance
recycling is established, disposal takes place via the
With few exceptions, all products have a five-year waste incineration plant.
warranty. Furthermore, an after-sale service warranty
of 15 years is provided. 2.16 Further information
2.13 Extraordinary effects Additional information about our products can be found
at https://www.hansgrohe.com.
Fire
3. LCA: Calculation rules
3.1 Declared Unit
The results of this EPD are valid for the following
functional unit: 3.2 System boundary
Provide sanitary function for one (1) average kitchen This representative EPD follows the EPD type "cradle
faucet unit used in accordance with the manufacturer's to gate - with options". The following life cycle modules
recommendations for a 10-year life, following the are declared:
manufacturer's operating instructions. An average Modules A1-A3:
conditioned kitchen faucet is considered the baseline The product stage begins with considering the
flow. production of the necessary raw materials and
energies, including all corresponding upstream chains
Weighted averaging based on production tonnages in and the actual procurement transports. Furthermore,
2021 is chosen as basis for creating the environmental the entire manufacturing phase was mapped, including
profile. 133 different kitchen faucets were considered. the treatment of production waste until the end-of-
waste status (EoW) was reached. Green electricity
Functional unit from hydropower is used for the manufacturing
Name Value Unit processes in Germany. US electricity mix is used for
Declared unit 1 pce. the US production site. Chinese electricity mix is used
Functional unit 1 pce. for the Chinese production site, although electricity
Functional unit with packaging 2.45 kg from photovoltaic is partly used there.
Packaging 0.48 kg Module A4:
Weight range of the products All distribution transports to the customers were
1.52 - 5.75 kg
examined considered.
Module A5:
4 Environmental Product Declaration Hansgrohe Group – Kitchen Faucets
This module covers the installation process with the datasets were only used when suitable GaBi datasets
corresponding packaging waste generated that needs were not available.
to be disposed.
Modules B1 & B3-B5: 3.6 Data quality
These modules were considered, but evaluated as not The background datasets used for accounting
relevant for the products and considered as zero. purposes mainly originate from the respective updated
Module B2: GaBi databases at the time of calculation. The data for
Maintenance expenses are declared in this module the examined products was captured on
and consist of weekly cleaning expense and cartridge the basis of evaluations of internal production and
replacement. environmental data, the collection of LCA relevant data
Module B6: within the supply chain, as well as the evaluation of
This module considers the energy input required to relevant data for the energy supply. The collected
bring water to a certain temperature for the use of a data were checked for plausibility and consistency.
gas low temperature boiler (scenario B6/1) and for the Good representativity can be assumed.
use of an electric instantaneous water heater (scenario
B6/2). For the assessment of the variability of the results, all
Module B7: products were balanced in addition to the average
This module considers the water consumption that can product. See at chapter 6 for explanation of the
be expected depending on the function of the product variability.
family.
Modules C1-C4: 3.7 Period under review
The modules include the environmental impacts for Life cycle assessment data were collected in 2021.
dismantling of the products and the treatment of the
waste fractions until the end-of-waste status (EoW) is 3.8 Allocation
reached, including the associated transports at the end For the production process nearly all raw materials,
of the product life cycle. precursors and supplies could be assigned to the
Module D: declared product. Energy, water, galvanization process
Identification of the benefits and costs of the product and production waste were assigned to the highest
outside the system boundary. For waste, paper and value of either the heaviest, lightest or most sold
plastics, these consist of energy credits from thermal product of the product group. No byproducts are
utilization (A3, A5 and C3) in the form of the average produced and no allocation is required.
European electricity mix or thermal energy from natural Some of the brass losses from brass processing in
gas. Recycling of paper, plastic and metal scrap module A3 are directly reused by Hansgrohe and are
results in credits of the respective raw materials for the modelled as a closed loop. Another part of the brass
primary material portion of the input. The loads of the losses (brass particles and dusts) is disposed of as
waste incineration and recycling processes are waste (without debits and credits).
assigned to the respective modules (A3, A5 and C3) Credits for plastics, paper and cardboard recycled in
and not to module D. A5 and metallurgical waste in C3 are credited in
module D.
3.3 Estimates and assumptions Credits for the energy recovery of incinerated
Energy and water consumption, material amount for production waste in A1-3, paper, cardboard and
coating as well as waste during production could only plastics in A5 and plastics and other materials in C3
be determined on concrete, existing products and not are credited in module D.
on the average product. The highest value of all inputs The loads for waste water treatment and waste
and outputs for energy, waste and coating of the top disposal of core sand, waste oil and hazardous waste
seller, the lightest and the heaviest product was used from the manufacturing phase are allocated to module
for the calculation of energy, water, waste and coating. A3.
For the incineration with energy recovery (thermal and Packaging:
electric) of waste, an r1 value of > 0.6 is assumed. The For paper and cardboard, recycling (91 %) and energy
net efficiency for the average waste incinerated is recovery (9 %) are considered on a pro rata basis. For
between 38 % and 44 %, depending on the type of plastic, a proportionate recycling (52 %), energy
waste respectively the disposal data set. recovery (48 %) considered, based on Eurostat.
Deconstructed product at the end of life:
3.4 Cut-off criteria Since the product is predominantly made of metal, it is
The effect associated with the neglected mass shares assumed that most of its metallic components are
is less than 5% of the effect categories per module. recycled. 95 % of the non-metallic components are
The minimum limit of 1% total mass and the use of incinerated with energy recovery and 5 % are disposed
renewable and nonrenewable primary energy is not in landfill. For the metal components, it is assumed that
exceeded. 90 % are sent for material recycling, 5 % for
incineration with energy recovery (C3) and 5 % are
3.5 Background data disposed in landfill (C4).
The LCA software GaBi 10.6 was used to model the
life cycle. The entire manufacturing process, as well as 3.9 Comparability
energy consumption, were modelled on the basis of Basically, a comparison or an evaluation of EPD data
manufacturer specific data. is only possible if all the data sets to be compared
However, generic background datasets were used for were created according to EN 15804 and the building
the upstream and downstream processes. The majority context, respectively the product-specific
of the background datasets used were taken from the characteristics of performance, are taken into account.
current version (2021.2) of
the GaBi database. Ecoinvent Version 3.6 (2019) The background database used is GaBi 10.6 in the
database version 2021.2
5 Environmental Product Declaration Hansgrohe Group – Kitchen Faucets
4. LCA: Scenarios and additional technical information
Characteristic product properties Name Value Unit
Information on biogenic carbon Water consumption 25.187 m3
Energy demand 1172 kWh
Information on describing the biogenic Carbon End of life (C1-C4)
Content at factory gate Name Value Unit
The biogenic carbon content was calculated based on Collected separately 1.967 kg
the factors from the Thünen Intitute. Recycling 1.479 kg
Name Value Unit Energy recovery 0.389 kg
Biogenic carbon content in 0.18 kg C Landfilling 0.098 kg
accompanying packaging
Reuse, recovery and/or recycling potentials (D),
relevant scenario information
The following technical information is a basis for the The energy generated from energy recovery as well as
declared modules. recycled materials are assigned to module D as
possible potentials or avoided loads in subsequent
Transport to the building site (A4) systems. Credits are only given for the primary portion
Name Value Unit of the inputs.
Transport distance (Truck) 731 km
Capacity utilisation (including
55 %
empty runs) (Truck)
Transport distance (Container
2454 km
Ship)
Capacity utilisation (Container
80 %
Ship)
Installation into the building (A5)
No additional resources or energy are required for the
installation. The packaging is disposed either by
recycling or incineration.
Name Value Unit
Packaging (Paper, cardboard and
0.481 kg
plastic)
Maintenance (B2)
For module B2, it is assumed that a weekly cleaning
of the product takes place, with 0.5 liter of water
containing 1.5% soap. The cartridge is replaced once
during its service life.
Name Value Unit
Number/R
Maintenance cycle (cleaning) 520
SL
Water consumption/Cycle weekly
0.5 Liter/cycle
(cleaning)
Soap concentration (cleaning) 1.5 %
Water consumption (cleaning) 0.26 m3
Auxiliary Soap/Tensides
3.9 kg
(cleaning)
Maintenance Cycle (cartridge Number/R
1
replacement) SL
Cartridge (cartridge replacement) 0.0581 kg/RSL
Service life
Hansgrohe SE declares a Service Life of 10 years as
an empirical value for the kitchen faucets when used in
accordance with the care instructions. This value is
based on their technical service centre's statistics on
service life in the market and complaints.
Name Value Unit
Life Span according to the
10 a
manufacturer
Operational energy use (B6) and Operational water
use (B7)
6 Environmental Product Declaration Hansgrohe Group – Kitchen Faucets
5. LCA: Results
The following table shows the result of the LCA for 1 piece of an average kitchen faucet. The results in the B-
module are based on a lifetime of 10 years. Scenario B6/1 shows the result for the use of a gas low temperature
boiler. Scenario B6/2 shows the result for the use of an electric instantaneous water heater.
DESCRIPTION OF THE SYSTEM BOUNDARY (X = INCLUDED IN LCA; ND = MODULE OR INDICATOR NOT
DECLARED; MNR = MODULE NOT RELEVANT)
BENEFITS AND
CONSTRUCTI LOADS
PRODUCT STAGE ON PROCESS USE STAGE END OF LIFE STAGE BEYOND THE
STAGE SYSTEM
BOUNDARIES
7 Environmental Product Declaration Hansgrohe Group – Kitchen Faucets
lairetam
waR
ylppus tropsnarT
gnirutcafunaM
eht
morf
tropsnarT
etis
eht
ot
etag
ylbmessA esU
ecnanetniaM
riapeR
tnemecalpeR tnemhsibrufeR
ygrene
lanoitarepO esu
retaw
lanoitarepO esu
noitcurtsnoc-eD
noitilomed tropsnarT
gnissecorp
etsaW
lasopsiD -esueR -yrevoceR -gnilcyceR laitnetop
A1 A2 A3 A4 A5 B1 B2 B3 B4 B5 B6 B7 C1 C2 C3 C4 D
X X X X X X X X X X X X X X X X X
RESULTS OF THE LCA - ENVIRONMENTAL IMPACT according to EN 15804+A2: 1 piece average kitchen
faucet incl. packaging
Core Indicator Unit A1-A3 A4 A5 B1 B2 B3 B4 B5 B6/1 B6/2 B7 C1 C2 C3 C4 D
-
5.98E+2.03E- 7.07E-0.00E+1.31E+0.00E+0.00E+0.00E+3.13E+4.67E+1.49E+0.00E+3.36E- 7.87E- 5.12E-
GWP-total [kg CO2-Eq.]
0 1 1 0 1 0 0 0 2 2 1 0 2 1 3
4.55E+
0
-
6.62E+2.02E- 5.00E-0.00E+1.01E+0.00E+0.00E+0.00E+3.13E+4.66E+1.49E+0.00E+3.33E- 7.87E- 5.12E-
GWP-fossil [kg CO2-Eq.]
0 1 2 0 1 0 0 0 2 2 1 0 2 1 3
3.90E+
0
-6.57E-0.00E+6.57E-0.00E+0.00E+0.00E+0.00E+0.00E+0.00E+0.00E+0.00E+0.00E+0.00E+0.00E+0.00E+-6.41E-
GWP-biogenic [kg CO2-Eq.]
1 0 1 0 0 0 0 0 0 0 0 0 0 0 0 1
1.40E- 1.24E- 9.08E-0.00E+3.01E+0.00E+0.00E+0.00E+1.58E- 6.59E- 1.21E-0.00E+2.73E- 9.20E- 4.95E--9.90E-
GWP-luluc [kg CO2-Eq.]
2 3 5 0 0 0 0 0 2 1 2 0 4 5 6 3
4.36E- 3.52E- 3.29E-0.00E+5.43E-0.00E+0.00E+0.00E+1.13E- 1.12E- 1.41E-0.00E+6.59E- 2.06E- 1.20E--4.39E-
ODP [kg CFC11-Eq.]
8 17 16 0 7 0 0 0 13 11 13 0 18 10 17 8
7.13E- 2.11E- 4.93E-0.00E+3.37E-0.00E+0.00E+0.00E+1.92E- 9.69E- 3.67E-0.00E+5.58E- 2.13E- 1.61E--4.74E-
AP [mol H+-Eq.]
2 3 5 0 2 0 0 0 1 1 2 0 5 4 5 2
8.67E- 4.63E- 9.55E-0.00E+2.91E-0.00E+0.00E+0.00E+2.85E- 1.25E- 1.59E-0.00E+9.92E- 1.51E- 2.03E--7.51E-
EP-freshwater [kg P-Eq.]
4 7 8 0 4 0 0 0 5 3 2 0 8 7 7 4
9.33E- 5.90E- 1.70E-0.00E+7.70E-0.00E+0.00E+0.00E+8.16E- 2.30E- 6.96E-0.00E+2.20E- 7.16E- 4.11E--5.30E-
EP-marine [kg N-Eq.]
3 4 5 0 3 0 0 0 2 1 2 0 5 5 6 3
1.01E- 6.51E- 2.02E-0.00E+9.18E-0.00E+0.00E+0.00E+8.91E-2.42E+1.10E-0.00E+2.51E- 9.38E- 4.36E--5.78E-
EP-terrestrial [mol N-Eq.]
1 3 4 0 2 0 0 0 1 0 1 0 4 4 5 2
2.77E- 1.60E- 4.25E-0.00E+3.06E-0.00E+0.00E+0.00E+2.38E- 6.25E- 2.81E-0.00E+4.98E- 1.90E- 1.28E--1.61E-
POCP [kg NMVOC-Eq.]
2 3 5 0 2 0 0 0 1 1 2 0 5 4 5 2
4.57E- 1.50E- 4.76E-0.00E+1.15E-0.00E+0.00E+0.00E+1.68E- 1.37E- 1.94E-0.00E+2.96E- 1.46E- 3.49E--3.89E-
ADPE [kg Sb-Eq.]
3 8 9 0 5 0 0 0 5 4 6 0 9 8 10 3
-
9.76E+2.64E+2.83E-0.00E+2.30E+0.00E+0.00E+0.00E+5.37E+8.29E+1.54E+0.00E+4.45E- 6.15E- 7.35E-
ADPF [MJ] 4.80E+
1 0 1 0 2 0 0 0 3 3 2 0 1 1 2
1
-
[m³ world-Eq 9.17E+1.49E- 1.06E-0.00E+3.49E+0.00E+0.00E+0.00E+8.20E-7.47E+4.59E+0.00E+3.10E- 7.81E--5.33E-
WDP 7.40E+
deprived] 0 3 2 0 0 0 0 0 1 1 0 0 4 2 5
0
GWP = Global warming potential; ODP = Depletion potential of the stratospheric ozone layer; AP = Acidification potential of land and water; EP =
Caption Eutrophication potential; POCP = Formation potential of tropospheric ozone photochemical oxidants; ADPE = Abiotic depletion potential for non-
fossil resources; ADPF = Abiotic depletion potential for fossil resources; WDP = Water (user) deprivation potential
RESULTS OF THE LCA - INDICATORS TO DESCRIBE RESOURCE USE according to EN 15804+A2: 1 piece
average kitchen faucet incl. packaging
Indicator Unit A1-A3 A4 A5 B1 B2 B3 B4 B5 B6/1 B6/2 B7 C1 C2 C3 C4 D
-
PERE [MJ] 1.81E+11.19E-17.85E+00.00E+04.72E+10.00E+00.00E+00.00E+04.67E+13.82E+34.52E+10.00E+02.56E-22.95E-15.34E-3
1.50E+1
-
PERM [MJ] 7.76E+00.00E+0 0.00E+00.00E+00.00E+00.00E+00.00E+00.00E+00.00E+00.00E+00.00E+00.00E+00.00E+00.00E+00.00E+0
7.76E+0
-
PERT [MJ] 2.59E+11.19E-19.15E-20.00E+04.72E+10.00E+00.00E+00.00E+04.67E+13.82E+34.52E+10.00E+02.56E-22.95E-15.34E-3
1.50E+1
-
PENRE [MJ] 8.54E+12.65E+01.11E+00.00E+02.30E+20.00E+00.00E+00.00E+05.37E+38.29E+31.54E+20.00E+04.46E-11.16E+17.35E-2
4.82E+1
-
PENRM [MJ] 1.24E+10.00E+0-8.26E-10.00E+00.00E+00.00E+00.00E+00.00E+00.00E+00.00E+00.00E+00.00E+00.00E+0 0.00E+00.00E+0
1.10E+1
-
PENRT [MJ] 9.78E+12.65E+02.83E-10.00E+02.30E+20.00E+00.00E+00.00E+05.37E+38.29E+31.54E+20.00E+04.46E-16.15E-17.35E-2
4.82E+1
SM [kg] 7.20E-10.00E+00.00E+00.00E+02.46E-30.00E+00.00E+00.00E+00.00E+00.00E+00.00E+00.00E+00.00E+00.00E+00.00E+01.28E+0
RSF [MJ] 0.00E+00.00E+00.00E+00.00E+00.00E+00.00E+00.00E+00.00E+00.00E+00.00E+00.00E+00.00E+00.00E+00.00E+00.00E+00.00E+0
NRSF [MJ] 0.00E+00.00E+00.00E+00.00E+00.00E+00.00E+00.00E+00.00E+00.00E+00.00E+00.00E+00.00E+00.00E+00.00E+00.00E+00.00E+0
FW [m³] 2.15E-11.37E-42.90E-40.00E+08.19E-20.00E+00.00E+00.00E+05.24E-23.72E+01.31E-10.00E+02.93E-51.94E-39.18E-7-1.67E-1
PERE = Use of renewable primary energy excluding renewable primary energy resources used as raw materials; PERM = Use of
Caption
renewable primary energy resources used as raw materials; PERT = Total use of renewable primary energy resources; PENRE = Use of
non-renewable primary energy excluding non-renewable primary energy resources used as raw materials; PENRM = Use of non-
renewable primary energy resources used as raw materials; PENRT = Total use of non-renewable primary energy resources; SM = Use
of secondary material; RSF = Use of renewable secondary fuels; NRSF = Use of non-renewable secondary fuels; FW = Use of net fresh
water
RESULTS OF THE LCA – WASTE CATEGORIES AND OUTPUT FLOWS according to EN 15804+A2:
1 piece average kitchen faucet incl. packaging
Indicator Unit A1-A3 A4 A5 B1 B2 B3 B4 B5 B6/1 B6/2 B7 C1 C2 C3 C4 D
1.12E- 5.83E- 2.35E- 1.76E- 1.30E-
HWD [kg] 1.40E-6 0.00E+04.25E-30.00E+00.00E+00.00E+01.00E-62.19E-63.16E-80.00E+0 -6.93E-6
10 11 11 10 11
NHWD [kg] 1.15E+03.80E-43.12E-30.00E+03.68E-10.00E+00.00E+00.00E+07.06E-15.88E+02.45E+10.00E+07.00E-52.43E-29.82E-2-8.57E-1
RWD [kg] 3.75E-34.37E-61.47E-50.00E+02.14E-30.00E+00.00E+00.00E+01.19E-21.23E+01.26E-20.00E+08.09E-74.28E-58.41E-7-2.52E-3
CRU [kg] 0.00E+00.00E+00.00E+00.00E+00.00E+00.00E+00.00E+00.00E+00.00E+00.00E+00.00E+00.00E+00.00E+00.00E+00.00E+00.00E+0
MFR [kg] 0.00E+00.00E+04.28E-10.00E+00.00E+00.00E+00.00E+00.00E+00.00E+00.00E+00.00E+00.00E+00.00E+01.48E+00.00E+00.00E+0
MER [kg] 0.00E+00.00E+00.00E+00.00E+09.01E-40.00E+00.00E+00.00E+00.00E+00.00E+00.00E+00.00E+00.00E+00.00E+00.00E+00.00E+0
EEE [MJ] 2.54E-20.00E+01.50E-10.00E+01.58E-10.00E+00.00E+00.00E+00.00E+00.00E+00.00E+00.00E+00.00E+03.20E-23.21E-40.00E+0
EET [MJ] 5.73E-20.00E+02.71E-10.00E+02.87E-10.00E+00.00E+00.00E+00.00E+00.00E+00.00E+00.00E+00.00E+06.00E-20.00E+00.00E+0
HWD = Hazardous waste disposed; NHWD = Non-hazardous waste disposed; RWD = Radioactive waste disposed; CRU = Components
Caption for re-use; MFR = Materials for recycling; MER = Materials for energy recovery; EEE = Exported electrical energy; EET = Exported
thermal energy
RESULTS OF THE LCA – additional impact categories according to EN 15804+A2-optional:
1 piece average kitchen faucet incl. packaging
Indicator Unit A1-A3 A4 A5 B1 B2 B3 B4 B5 B6/1 B6/2 B7 C1 C2 C3 C4 D
[Disease 3.27E- 0.00E+ 0.00E+ 0.00E+ 0.00E+ 0.00E+ 3.49E- 1.72E- -4.28E-
PM 6.84E-73.33E-8 1.66E-6 1.33E-68.17E-64.12E-7 1.46E-9
Incidence] 10 0 0 0 0 0 10 10 7
-
[kBq U235- 2.38E+ 0.00E+ 1.08E+ 0.00E+ 0.00E+ 0.00E+ 1.89E+ 2.03E+ 1.99E+ 0.00E+
IRP 6.36E-41.84E-3 1.18E-44.09E-31.20E-41.97E+
Eq.] 0 0 0 0 0 0 0 2 0 0
0
-
2.96E+ 1.95E+ 0.00E+ 1.02E+ 0.00E+ 0.00E+ 0.00E+ 7.34E+ 3.48E+ 2.17E+ 0.00E+
ETP-fw [CTUe] 1.48E-1 3.30E-15.04E-13.19E-21.38E+
2 0 0 2 0 0 0 1 3 3 0
2
3.86E- 4.46E- 0.00E+ 0.00E+ 0.00E+ 0.00E+ 0.00E+ 6.67E- 1.30E- 2.67E- -7.72E-
HTP-c [CTUh] 7.76E-8 1.61E-8 1.57E-89.87E-87.36E-8
11 12 0 0 0 0 0 12 11 12 9
2.08E- 0.00E+ 0.00E+ 0.00E+ 0.00E+ 0.00E+ 3.55E- 7.39E- 2.58E- -2.82E-
HTP-nc [CTUh] 4.68E-72.00E-9 3.82E-7 1.66E-63.72E-67.57E-6
10 0 0 0 0 0 10 10 10 7
-
4.95E+ 0.00E+ 1.59E+ 0.00E+ 0.00E+ 0.00E+ 3.13E+ 2.61E+ 7.58E+ 0.00E+
SQP [-] 6.98E-11.05E-1 1.53E-12.44E-15.39E-34.40E+
1 0 2 0 0 0 1 3 1 0
1
PM = Potential incidence of disease due to PM emissions; IR = Potential Human exposure efficiency relative to U235; ETP-fw = Potential
Caption comparative Toxic Unit for ecosystems; HTP-c = Potential comparative Toxic Unit for humans (cancerogenic); HTP-nc = Potential
comparative Toxic Unit for humans (not cancerogenic); SQP = Potential soil quality index
Disclaimer 1 – for the indicator “Potential Human exposure efficiency relative to U235”.
This impact category deals mainly with the eventual impact of low dose ionizing
radiation on human health of the nuclear fuel cycle. It does not consider effects due to possible
nuclear accidents, occupational exposure nor due to radioactive waste disposal in underground
facilities. Potential ionizing radiation from the soil, from radon and from some construction materials is also not
measured by this indicator.
Disclaimer 2 – for the indicators “abiotic depletion potential for non-fossil resources”, “abiotic depletion potential
for fossil resources”, “water (user) deprivation potential, deprivation-weighted water consumption”, “potential
comparative toxic unit for ecosystems”, “potential comparative toxic unit for humans – cancerogenic”, “Potential
comparative toxic unit for humans - not cancerogenic”, “potential soil quality index”.
The results of this environmental impact indicator shall be used with care as the
uncertainties on these results are high or as there is limited experienced with the indicator.
6. LCA: Interpretation
8 Environmental Product Declaration Hansgrohe Group – Kitchen Faucets
The dominance analysis shows that modules B2, B6 basic structure of the product types is always similar.
and B7 are the dominant life cycle stages in most of Material type and quantity proportions do not differ
the categories. The contribution of B2 is due to the much, as also shown in the average material
demand of soap and water for cleaning. Module B6 composition table.
dominates most of the indicators due to the energy The deviation of the GWP fossil in modules A1-C4 has
demand for water heating and module B7 has a high a maximum of 48% and a minimum of -54% with
contribution to EPfreshwater due to the wastewater scenario B6/1 (gas low temperature boiler). The
treatment. The module A1-A3 has a very low deviation of the GWP fossil in modules A1-C4 has a
contribution to all categories except of ADPE. In this maximum of 45% and a minimum of -50% with
indicator the provision of brass and zinc has the largest scenario B6/2 (electric instantaneous water heater).
contribution. The end-of-life stage has no significant For an average scenario, where 50% of water is
influence on the environmental indicators. heated with gas low temperature boiler and 50% with
The environmental burdens from the transports electric instantaneous water heater, 63% of the kitchen
(modules A4 and C2) account for less than 1% of the faucets produced are above the average GWP fossil
total burdens of the respective indicators in all cases. value. Whereas 37% reflect the average or are lower
The possible potentials of avoided loads of subsequent than the average. However, 92% of the ones which are
systems (module D) lie outside the considered system above the average just deviate between +4 and +13
boundaries and relate exclusively to credits from %.
recycling and thermal recycling by means of Modules B6 and B7 account for more than 90% of the
incineration with energy recovery of the different GWP indicator. The deviation from the average is
materials. mainly caused by the flow rate in module B7. The
731,675 kitchen faucets of 133 different product types deviation from the average is mainly caused by the
were produced. For the assessment of the variability of flow rate in module B7. The higher the deviation from
the results, all products were balanced and compared the average GWP, the higher the flow rate. The flow
to the average product weighted by production volume. rate ranges between 4.6 and 16 l/min. Consequently,
The different types of products all have the same the production phase has a minor influence on the LCA
function and differ mainly in terms of design, which has results.
an influence on construction and materials used. The
7. Requisite evidence
The drinking water regulation determines the quality of - Part A – Procedure for the acceptance
drinking water at the point of withdrawal. This result in - Part B – 4MS Common Composition List
requirements for used materials in drinking water  Metal recommendation of the federal
installations in general and therefore in sanitary fittings environment agency: metal materials suitable
in particular.
for drinking water hygiene
All materials used by Hansgrohe SE, which are in
contact with drinking water, fulfill the drinking water
regulation. Regulations for other materials (Germany):
Regulations for metals (Europe-wide):  KTW: Assessment basis for plastics and other
 Acceptance of metallic materials used for organic materials in contact with drinking
products in contact with drinking water: 4MS water
Common Approach  Elastomer guideline: Guideline for the
9 Environmental Product Declaration Hansgrohe Group – Kitchen Faucets
hygienic assessment of elastomers in contact drinking water (sanitary lubricants), (Lubricant
with drinking water Guideline)
 Thermoplastic elastomers: Recommendation
for the hygienic assessment of products made Regulation for other materials (France):
of thermoplastic elastomers in contact with  ACS: Attestation de Conformité Sanitaire
drinking water (TPE transition (plastics, elastomers, metals)
recommendation)
 Ceramics: draft assessment basis for Regulation for other materials (UK):
enamels and ceramic materials: assessment  BS 69 20: Suitability of non-metallic products
basis for enamels and ceramic materials in for use in contact with water intended for
contact with drinking water (enamel/ceramic human consumption with regard to their effect
assessment basis) on the quality of water (plastics, elastomers)
 Lubricants: Guideline for the hygienic
assessment of lubricants in contact with Products of the Hansgrohe SE are therefore uncritical
to use with any drinking water.
8. References
Standards declarations - Core rules for the product category of
construction products
EN 200
EN 200:2008: Sanitary tapware – Single taps and DIN EN ISO 45001
combination taps for water supply systems of type 1 DIN EN ISO 45001:2018: Occupational health and
and type 2 safety management systems — Requirements with
guidance for use. 2018-03
EN 816
EN 816:2017: Sanitary tapware – Automatic shut-off DIN EN ISO 50001
valves PN 10 DIN EN ISO 50001:2018: Energy management
systems — Requirements with guidance for use. 2018-
EN 817 08
EN 817:2008: Sanitary tapware – Mechanical mixing
valves (PN 10) Further References
ISO 3822 AVV
ISO 3822: Acoustics – Laboratory tests on noise Draft General administrative provision relating to the
emission from appliances and equipment used in water Order on the European list of wastes (Waste List Order
supply installations – German designation: AVV) of 10 December 2001.
DIN 4102-1 ECHA
DIN 4102-1: Fire behaviour of building materials and European Chemicals Agency (ECHA) Candidate List of
building components - Part 1: Building materials; Substances of Very High Concern (SVHC) for
concepts, requirements and tests. 1998-05 Authorisation https://echa.europa.eu/de/candidate-
listtable
DIN EN ISO 9001
DIN EN ISO 9001:2015: Quality management systems Ecoinvent
- Requirements (ISO 9001:2015) ecoinvent 3.6 Database on Life Cycle Inventories (Life
Cycle Inventory data), ecoinvent Association, Zürich,
DIN EN 13501-1 2020
DIN EN 13501-1:2019-05: Fire classification of
construction products and building elements - Part 1: EU Ordinance on biocide Products No. 528/2012
Classification using data from reaction to fire tests; European Parliament, 2012. Regulation (EU) no
German version EN 13501-1:2018 528/2012 of the European parliament and of the
council of 22 May 2012 concerning the making
DIN EN ISO 14001 available on the market and use of biocidal products
DIN EN ISO 14001:2015, Environmental management
systems — Requirements with guidance for use, 2015- Eurostat
09 Eurostat, last update 26/10/2021 on
https://ec.europa.eu/eurostat/databrowser/view/ten000
DIN EN ISO 14025 63/default/table?lang=en
DIN EN ISO 14025: Environmental labels and
declarations - Type III environmental declarations - GaBi
Principles and procedures, 2011-10 GaBi 10.6, GaBi Software System and Database for
Life Cycle Engineering version 2021.2, Sphera
EN 15804 Solutions GmbH, Leinfelden-Echterdingen, 1992-2021
DIN EN 15804:2012+A2:2019+AC:2021: Sustainability
of construction works - Environmental product IBU 2021
General Instructions for the EPD programme of Institut
10 Environmental Product Declaration Hansgrohe Group – Kitchen Faucets
Bauen und Umwelt e.V. Version 2.0, Berlin: Institut on the EPD for fittings and showers. Version 1.1,
Bauen und Umwelt e.V., 2021, www.ibu-epd.com Berlin, 03/2022
PCR Part A Thünen Institute
Institut Bauen und Umwelt e.V. (IBU), Product Diestel, Sylvia / Weimar, Holger: Der Kohlenstoffgehalt
Category Rules for Building-Related Products and in Holz- und Papierprodukten - Herleitung und
Services. Part A: Calculation rules for the life cycle Umrechnungsfaktoren. Thünen Working Paper 38.
assessment and requirements on the project report. Johann Heinrich von Thünen-Institut. Hamburg, 2014
Version 2.1, Berlin, 11/2021
PCR Part B
Institut Bauen und Umwelt e.V. (IBU), Requirements
11 Environmental Product Declaration Hansgrohe Group – Kitchen Faucets
Publisher
Institut Bauen und Umwelt e.V. Tel +49 (0)30 3087748- 0
Hegelplatz 1 Fax +49 (0)30 3087748- 29
10117 Berlin Mail info@ibu-epd.com
Germany Web www.ibu-epd.com
Programme holder
Institut Bauen und Umwelt e.V. Tel +49 (0)30 - 3087748- 0
Hegelplatz 1 Fax +49 (0)30 – 3087748 - 29
10117 Berlin Mail info@ibu-epd.com
Germany Web www.ibu-epd.com
Author of the Life Cycle
Assessment Tel +49 421 70 90 84 33
brands & values GmbH Fax +49 421 70 90 84 35
Altenwall 14 Mail info@brandsandvalues.com
28195 Bremen Web www.brandsandvalues.com
Germany
Owner of the Declaration
Hansgrohe Group Tel +49 7836 51-0
Auestr. 5-9 Fax +49 7836 51-1300
77761 Schiltach Mail info@hansgrohe-group.com
Germany Web http://www.hansgrohe-
group.com
