ENVIRONMENTAL PRODUCT DECLARATION
as per ISO 14025 and EN 15804+A1
Owner of the Declaration ArcelorMittal Europe
Programme holder Institut Bauen und Umwelt e.V. (IBU)
Publisher Institut Bauen und Umwelt e.V. (IBU)
Declaration number EPD-ARM-20210338-CBB1-EN
Issue date 13.04.2022
Valid to 12.04.2027
Reinforcing steel in Bars (Rebars)
ArcelorMittal Europe
www.ibu-epd.com | https://epd-online.com
Umwelt Produktdeklaration Name des Herstellers – Name des Produkts
General Information
ArcelorMittal Europe Reinforcing steel
Programme holder Owner of the declaration
IBU – Institut Bauen und Umwelt e.V. ArcelorMittal Europe-Long Products
Panoramastr. 1 66, rue de Luxembourg
10178 Berlin L-4221 Esch-sur-Alzette
Germany Luxembourg
Declaration number Declared product / declared unit
EPD-ARM-20210338-CBB1-EN 1 metric ton of Reinforcing steel.
This declaration is based on the product Scope:
category rules: The declaration applies to 1 metric ton of Reinforcing
Reinforcing Steel, 11.2017 steel produced by ArcelorMittal.
(PCR checked and approved by the SVR)
The Life Cycle Assessment is based on annual data
Issue date collected from the plants involved in the production:
13.04.2022 Warsaw in Poland and Hamburg in Germany.
Valid to The owner of the declaration shall be liable for the
12.04.2027 underlying information and evidence; the IBU shall not
be liable with respect to manufacturer information, life
cycle assessment data and evidences.
The EPD was created according to the specifications
of EN 15804+A1. In the following, the standard will be
simplified as EN 15804.
Verification
The standard EN 15804 serves as the core PCR
Independent verification of the declaration and data
according to ISO 14025:2010
Dipl. Ing. Hans Peters internally x externally
(chairman of Institut Bauen und Umwelt e.V.)
Dr. Alexander Röder Matthias Klingler
(Managing Director Institut Bauen und Umwelt e.V.)) (Independent verifier)
Product
Product description/Product definition concrete - Weldable reinforcing steel - General
This EPD applies to 1 metric ton of steel for the The CE-marking takes into account the proof of
reinforcement of concrete according to EN 10080 conformity with the respective harmonised standards
standard (as weldable reinforcing steel in bars and based on the legal provisions above.
coils), which is obtained from scrap and direct reduced
iron (DRI) melted in Electric Arc Furnace, followed by For the application and use the respective national
hot rolling process and cold working, where provisions apply.
appropriate.
Application
Reinforcing Steel, also called rebar (including standard
rebars, special rebars – Krybar®, rock bolt, tie bars Rebars are steel rods that are used as a tension
and threaded bars) covers carbon steel for device in concrete. Typical applications are in the
geotechnical use and the reinforcement of concrete. construction of buildings, bridges, roads and other civil
The surface of rebars is patterned to form a better works (infrastructures, superstructures, etc.) as well as
bond with soil and concrete, in addition the ribs on mining.
threaded bars, rock bolts and tie bars allow for bolting.
Technical Data
For the placing on the market in the European
Union/European Free Trade Association (EU/EFTA) This EPD is valid for Reinforcing steel of various steel
(with the exception of Switzerland) the following legal grades and different forms of delivery.
provisions apply: Performance data of the product in accordance with
the Declaration of Performance.
EN 10080:2005, Steel for the reinforcement of
2 Environmental Product Declaration ArcelorMittal – Reinforcing steel
Base materials/Ancillary materials
Constructional data
The base material of Reinforcing steel is iron. Alloying
elements are added in the form of ferroalloys or metals
Name Value Unit (most common elements are Manganese and Silicon).
Density 7850 kg/m3 Some small quantities of other elements may be
Modulus of elasticity 210000 N/mm2 present in the steel.
Coefficient of thermal expansion 12 10-6K-1
Thermal conductivity 48 W/(mK) No substances listed on the “Candidate List of
Melting point 1536 °C Substances of Very High Concern for Authorisation” by
Minimum yield strength 460 - 900 N/mm2 the European Chemicals Agency EC 1907-2006 are
Tensile strength 483 - 1100 N/mm2 contained in the steel in declarable quantities.
Type of steel Bar -
This product contains substances listed in the
EAF and
Production route - candidate list (date: 22.2.2021) exceeding 0.1
DRI-EAF
percentage by mass: no
Shear modulus 81000 N/mm²
Reference service life
Product not harmonised in accordance with the CPR
A reference service life for Reinforcing steel is not
but in accordance with other provisions for
declared. These are construction products with many
harmonisation of the EU, such as EN 10080.
different applications purposes. The lifetime therefore
will be limited by the service life of the work.
For the application and use the respective national
provisions apply, as well as normally used standards
such as (not exhaustive list): EN 1992-1-1, EN 1992-1-
2, EN 1992-2, EN 1992-3, DIN 488-1 and BS4449.
LCA: Calculation rules
Declared Unit thus becoming input to the product system in
the inventory.
The declaration refers to the declared unit of 1 metric
ton of Reinforcing steel as specified in Part B
requirements on the EPD for reinforcing steel.
Modules C3-C4 take into account the sorting and
shredding of after-use steel, as well as the
Foreground data for the production are integrated into
nonrecovered scrap due to sorting efficiency which is
the software model for the considered production
landfilled. A conservative value of 10% landfill is
site/company. The LCI is assessed as per the annual
considered.
production data of ArcelorMittal Europe at the sites
Warszawa (Poland) and Hamburg (Germany). The
Module D refers to the End-of-Life, including recycling.
background data are taken from GaBi Documentation.
Comparability
Declared unit
Basically, a comparison or an evaluation of EPD data
is only possible if all the data sets to be compared
Name Value Unit
were created according to EN 15804 and the building
Declared unit 1 t
context, respectively the product-specific
Density 7850 kg/m3
characteristics of performance, are taken into account.
For the life cycle modelling of the product under study,
the GaBi Software System for Life Cycle Engineering,
System boundary
content version 2021.2, is used (GaBi).
Type of the EPD: cradle-to-gate - with options.
Module A1-A3, Modules C3-C4 and Module D were
considered.
Modules A1-A3 include the following:
 The provision of resources, additives, and
energy
 Transport of resources and additives to the
production site
 Production processes on-site including
energy, production of additives, disposal of
production residues, and consideration of
related emissions
 Recycling of production/manufacturing scrap.
Steel scrap is assumed to reach the end-of-
waste status once it is shredded and sorted,
3 Environmental Product Declaration ArcelorMittal – Reinforcing steel
LCA: Scenarios and additional technical information
Current practice for the average rebar product consists
of 91 % recycling, 1 % reuse and 8 % landfill according
to SteelConstruction-info.
This EPD considers as a conservative approach 90%
recycling and 10 % landfill:
End of life (C3 - C4)
Name Value Unit
Landfilling 10 %
Reuse, recovery and/or recycling potentials (D),
relevant scenario information
Name Value Unit
Recycling 90 %
4 Environmental Product Declaration ArcelorMittal – Reinforcing steel
LCA: Results
DESCRIPTION OF THE SYSTEM BOUNDARY (X = INCLUDED IN LCA; MND = MODULE NOT DECLARED;
MNR = MODULE NOT RELEVANT)
BENEFITS AND
CONSTRUCTI LOADS
PRODUCT STAGE ON PROCESS USE STAGE END OF LIFE STAGE BEYOND THE
STAGE SYSTEM
BOUNDARIES
5 Environmental Product Declaration ArcelorMittal – Reinforcing steel
lairetam
waR
ylppus tropsnarT
gnirutcafunaM
eht
morf
tropsnarT
etis
eht
ot
etag
ylbmessA esU
ecnanetniaM
riapeR
tnemecalpeR tnemhsibrufeR
ygrene
lanoitarepO esu
retaw
lanoitarepO esu
noitcurtsnoc-eD
noitilomed tropsnarT
gnissecorp
etsaW
lasopsiD -esueR -yrevoceR -gnilcyceR laitnetop
A1 A2 A3 A4 A5 B1 B2 B3 B4 B5 B6 B7 C1 C2 C3 C4 D
X X X MND MND MND MND MNR MNR MNR MND MND MND MND X X X
RESULTS OF THE LCA - ENVIRONMENTAL IMPACT according to EN 15804+A1: 1 ton reinforcing steel
Parameter Unit A1-A3 C3 C4 D
Global warming potential [kg CO2-Eq.] 8.18E+2 1.60E+0 1.43E+0 4.11E+2
Depletion potential of the stratospheric ozone layer [kg CFC11-Eq.] 2.15E-12 4.69E-14 7.83E-15 1.37E-12
Acidification potential of land and water [kg SO2-Eq.] 1.65E+0 2.99E-3 8.57E-3 6.40E-1
Eutrophication potential [kg (PO4)3--Eq.] 1.56E-1 4.48E-4 9.72E-4 4.63E-2
Formation potential of tropospheric ozone photochemical
[kg ethene-Eq.] 1.33E-1 2.60E-4 6.58E-4 1.91E-1
oxidants
Abiotic depletion potential for non-fossil resources [kg Sb-Eq.] 8.90E-5 4.70E-7 1.44E-7 1.07E-3
Abiotic depletion potential for fossil resources [MJ] 8.43E+3 1.82E+1 1.95E+1 4.25E+3
RESULTS OF THE LCA - INDICATORS TO DESCRIBE RESOURCE USE according to EN 15804+A1: 1 ton
reinforcing steel
Parameter Unit A1-A3 C3 C4 D
Renewable primary energy as energy carrier [MJ] 5.12E+2 1.22E+1 2.70E+0 -2.65E+2
Renewable primary energy resources as material utilization [MJ] 0.00E+0 0.00E+0 0.00E+0 0.00E+0
Total use of renewable primary energy resources [MJ] 5.12E+2 1.22E+1 2.70E+0 -2.65E+2
Non-renewable primary energy as energy carrier [MJ] 9.07E+3 2.82E+1 2.01E+1 4.22E+3
Non-renewable primary energy as material utilization [MJ] 0.00E+0 0.00E+0 0.00E+0 0.00E+0
Total use of non-renewable primary energy resources [MJ] 9.07E+3 2.82E+1 2.01E+1 4.22E+3
Use of secondary material [kg] 1.15E+3 0.00E+0 0.00E+0 0.00E+0
Use of renewable secondary fuels [MJ] 0.00E+0 0.00E+0 0.00E+0 0.00E+0
Use of non-renewable secondary fuels [MJ] 0.00E+0 0.00E+0 0.00E+0 0.00E+0
Use of net fresh water [m³] 1.48E+0 1.18E-2 4.95E-3 2.74E+1
RESULTS OF THE LCA – WASTE CATEGORIES AND OUTPUT FLOWS according to EN 15804+A1:
1 ton reinforcing steel
Parameter Unit A1-A3 C3 C4 D
Hazardous waste disposed [kg] 1.03E-6 6.99E-9 2.13E-9 -9.22E-7
Non-hazardous waste disposed [kg] 2.91E+0 1.89E-2 1.00E+2 -5.38E+1
Radioactive waste disposed [kg] 2.16E-1 3.89E-3 2.10E-4 -4.57E-4
Components for re-use [kg] 0.00E+0 0.00E+0 0.00E+0 0.00E+0
Materials for recycling [kg] 0.00E+0 9.00E+2 0.00E+0 0.00E+0
Materials for energy recovery [kg] 0.00E+0 0.00E+0 0.00E+0 0.00E+0
Exported electrical energy [MJ] 0.00E+0 0.00E+0 0.00E+0 0.00E+0
Exported thermal energy [MJ] 0.00E+0 0.00E+0 0.00E+0 0.00E+0
Note: 1153,8 kg of scrap are used in the manufacturing of 1 metric ton of rebar. After use, 900 kg steel are
recycled, and 100 kg are landfilled. The potential environmental impact calculated for module D depends on the
net amount of scrap left in the system, which is 900-1153,8 = -253,8 kg. This means that the system has a net
consumption of 253,8 kg of scrap. This is shown in module D as an environmental burden.
References
Standards: DIN 488-1:2009, Reinforcing steels - Part 1: Grades,
properties, marking
BS 4449
BS 4449:2005+A3:2016; Steel for the reinforcement of EN 10080
concrete. Weldable reinforcing steel. Bar, coil and EN 10080:2005, Steel for the reinforcement of
decoiled product. Specification concrete - Weldable reinforcing steel - General
DIN 488 EN 1992-1-1
EN 1992-1-1:2004, Eurocode 2: Design of concrete
structures - Part 1-1: General rules and rules for GaBi
buildings GaBi dataset documentation for the GaBi Software
System and Database for Life Cycle Engineering,
EN 1992-1-2 thinkstep AG, Leinfelden-Echterdingen, 2021
EN 1992-1-2:2004, Eurocode 2: Design of concrete (http://documentation.gabi-software.com/)
structures - Part 1-2: General rules - Structural fire
design IBU 2021
General Instructions for the EPD programme of Institut
EN 1992-2 Bauen und Umwelt e.V. Version 2.0, Berlin:
EN 1992-2:2005, Eurocode 2 - Design of concrete Institut Bauen und Umwelt e.V., 2021.
structures - Concrete bridges - Design and detailing www.ibuepd.com
rules
PCR Part A
EN 1992-3 PCR - Part A: Calculation rules for the Life Cycle
EN 1992-3:2006, Eurocode 2 - Design of concrete Assessment and Requirements on the Background
structures - Part 3: Liquid retaining and containment Report, version 1.8, Institut Bauen und Umwelt e.V.,
structures www.bau-umwelt.com, 2019
EN 15804 PCR Part B
EN 15804:2012-04+A1 2013, Sustainability of PCR – Part B: Requirements of the EPD for Metal
construction works — Environmental Product Ceilings, Institut Bauen und Umwelt e.V., www.bau-
Declarations — Core rules for the product category of umwelt.com, 2019
construction products.
SteelConstruction-info
ISO 14025 https://www.steelconstruction.info/The_recycling_and_
DIN EN ISO 14025:2011-10, Environmental labels and reuse_survey
declarations — Type III environmental declarations —
Principles and procedures. Worldsteel 2011
Life cycle assessment (LCA) methodology report
Other References: http://www.worldsteel.org/publications/
Candidate list - REACH
Regulation (EC) No 1907/2006 of the European
Parliament and of the Council on the Registration,
Evaluation, Authorisation and Restriction of Chemicals
(REACH). https://echa.europa.eu/candidate-list-table
6 Environmental Product Declaration ArcelorMittal – Reinforcing steel
Publisher
Institut Bauen und Umwelt e.V. Tel +49 (0)30 3087748- 0
Panoramastr. 1 Fax +49 (0)30 3087748- 29
10178 Berlin Mail info@ibu-epd.com
Germany Web www.ibu-epd.com
Programme holder
Institut Bauen und Umwelt e.V. Tel +49 (0)30 - 3087748- 0
Panoramastr 1 Fax +49 (0)30 – 3087748 - 29
10178 Berlin Mail info@ibu-epd.com
Germany Web www.ibu-epd.com
Author of the Life Cycle
Assessment Tel +49 711 341817-0
Sphera Solutions GmbH Fax +49 711 341817-25
Hauptstraße 111- 113 Mail info@sphera.com
70771 Leinfelden-Echterdingen Web www.sphera.com
Germany
Owner of the Declaration
ArcelorMittal Europe – Long Tel +352 5313 2142
Products – Bars & Rods Fax -
Rue de Luxemburg 66 Mail
4221 Esch-sur-Alzette longeurope.barsandrods@arcelo
Luxembourg rmittal.com
Web barsandrods.arcelormittal.com
