ENVIRONMENTAL PRODUCT DECLARATION
as per ISO 14025 and EN 15804+A2
Owner of the Declaration voestalpine AG
Publisher Institut Bauen und Umwelt e.V. (IBU)
Programme holder Institut Bauen und Umwelt e.V. (IBU)
Declaration number EPD-VOE-20230104-IBC2-EN
Issue date 09.05.2023
Valid to 08.05.2028
Annealed wire rod
voestalpine Wire Rod Austria GmbH
www.ibu-epd.com | https://epd-online.com
1. General Information
voestalpine Wire Rod Austria GmbH Annealed wire rod
Programme holder Owner of the declaration
IBU – Institut Bauen und Umwelt e.V. voestalpine AG
Hegelplatz 1 voestalpine-Straße 3
10117 Berlin 4020 Linz
Germany Austria
Declaration number Declared product / declared unit
EPD-VOE-20230104-IBC2-EN 1 tonne of annealed wire rod
This declaration is based on the product category rules: Scope:
Structural steels, 01.08.2021 This EPD is based on a declared unit of 1 metric tonne of average
(PCR checked and approved by the SVR) voestalpine annealed wire rod produced at the production site in St. Peter
Freienstein (Austria).
The owner of the declaration shall be liable for the underlying information
Issue date and evidence; the IBU shall not be liable with respect to manufacturer
information, life cycle assessment data and evidences.
09.05.2023
The EPD was created according to the specifications of EN 15804+A2. In
the following, the standard will be simplified as EN 15804.
Valid to
08.05.2028 Verification
The standard EN 15804 serves as the core PCR
Independent verification of the declaration and data according to ISO
14025:2011
internally X externally
Dipl.-Ing. Hans Peters
(Chairman of Institut Bauen und Umwelt e.V.)
Florian Pronold Prof. Dr. Birgit Grahl,
(Managing Director Institut Bauen und Umwelt e.V.) (Independent verifier)
1 Environmental Product Declaration - voestalpine Wire Rod Austria GmbH - Annealed wire rod
2. Product
2.1 Product description/Product definition
Wire rod made by voestalpine in St. Peter Freienstein is the
base product for lots of applications, that require un- or low
alloyed steel in round shape. Wire rod is hot rolled in
dimensions from 5 to 52 mm.
A large part of the produced wire rod is delivered to
voestalpines' own drawing facilities Wire Austria, Wire
Germany, Wire Italy and Special Wire for further processing.
Many customers use wire rod directly to manufacture finished-
The standard product range of voestalpine Wire Rod Austria
or semi-finished products.
contains around 500 different steel grades and a total number
of 3500 grades can be produced on customers' demands.
After the rolling process, wire rod can be heat treated in
annealing furnaces to achieve better deformation- and
Performance data of the product with respect to its
mechanical properties. The heat treatment is considered in this
characteristics in accordance with the relevant technical
EPD.
provision (no CE-marking).
For the use and application of the product the respective 2.4 Delivery status
national provisions at the place of use apply, in Germany for
The produced wire rod has a standard diameter range between
example the building codes of the federal states and the
5 and 52 mm. By applying the EN 10108 standard, tight
corresponding national specifications.
tolerances are guaranteed. Due to our state-of-the-art rolling
technologies, even stricter tolerances are achieved.
2.2 Application
Wire rod from voestalpine Wire Rod Austria GmbH is used for a
Delivery Condition acc. to EN 10027:
variety of applications.
The main amount is used for cold heading products. • +U +AC (annealed on spheroidised carbide)
Typical examples are fasteners, bolts and rivets, ball studs,
2.5 Base materials/Ancillary materials
high-strength screws and highly loaded shafts for automotive
lightweight construction. Further important products made out 100 % of the pre-material for the wire rod rolling process is
of wire rod are springs, bearings,chains, as well as welding made by voestalpine Stahl Donawitz GmbH, which is located
wire. right next to the wire rod rolling mill. The maximum alloyment
content is around 5 %.
Un- and low-alloyed steel grades categories:
The steel is produced by one of the two blast furnaces using
• Cold forging steel
the Linz-Donawitz-process (oxygen converter), which was
• Spring steel
developed by voestalpine in 1949.
• Chain steel
• Bearing steel
The steel works from voestalpine in Donawitz uses
• Soft drawing steel
approximately 20 % - 30 % of scrap (internal and external) for
• Saw wire
its steel production.
• Prestressing wire
• Machining steel
Depending on the steel grade and application the liquid steel is
• Welding wire
poured into one of the two continuous casting lines of
• Cold-work steel
voestalpine Stahl Donawitz and rolled over to a square billet
Market Segments:
format of 150 mm x 150 mm.
• Automotive
• Construction Each billet has a length up to approximately 18 m, a weight up
• Mechanical Engineering to 3 tonnes and is transported to the wire rod mill by train.
• Energy
• White goods This product/article/at least one partial article contains
• others substances listed in the candidate list (date: 16.1.2020)
exceeding 0.1 percentage by mass: no.
2.3 Technical Data
This EPD applies to all wire rod in the condition 'annealed' from This product/article/at least one partial article contains other
voestalpine Wire Rod Austria GmbH, which is why a general carcinogenic, mutagenic, reprotoxic (CMR) substances in
statement about mechanical properties is not possible. The categories 1A or 1B which are not on the candidate list,
technical data given for the products are generic literature data exceeding 0.1 percentage by mass: no.
for steel as described e.g. in Key to Steel. No product-specific
test rules are applicable to the data given: Biocide products were added to this construction product, or it
has been treated with biocide products (this then concerns a
Constructional data treated product as defined by the (EU) Ordinance on Biocide
Products No. 528/2012): no.
2.6 Manufacture
2 Environmental Product Declaration - voestalpine Wire Rod Austria GmbH - Annealed wire rod
The billets from voestalpine Stahl Donawitz GmbH are heated
up in the walking beam furnace to reach the required rolling For surface treated material it is possible to use wooden frames
temperature. on the truck to ensure a secure transport.
For dimensions up to 23 mm the loop-laying head and cooling This EPD considers steel bands as packaging. The majority of
conveyor line is used. The bar in coil line is used to produce products is delivered without additional packaging.
dimensions from 24 mm to 52 mm.
Coil dimensions:
A total number of 36 rolling stands, deform the wire rod to its
• Inner diameter ~ 850 mm
final dimension. Waterboxes along the rolling lines ensure that
• Outer diameter ~ 1250 mm
the required rolling temperatures are achieved.
• Length ~ 2 x 1200 mm or 1 x 2400 mm
• Weight: ~ 2 x 1,5 t or 1 x 3 t
After the rolling process, the wire rod is pickled in hydrochloric
acid to remove scale. 2.10 Condition of use
The following heat treatment (annealing) takes place in a bell- There is no change in material composition over the service life
type annealing furnace with a capacity of 48 t, temperatures of the product. If used as intended, no effects on the
around 700 °C and times up to ~24 hours. environment are to be expected.
Depending on customer requirements, voestalpine Wire Rod 2.11 Environment and health during use
Austria can apply 43 different annealing programs on the wire During the use of wire rod products, no effects on human and
rod depending on the diameter and steel grade. The goal is to animal health and no harmful emissions to air, soil and water
achieve a spherodized carbide structure on the wire rod to are expected.
optimize its deformation capability.
2.12 Reference service life
2.7 Environment and health during manufacturing Due to the variety of applications and their stresses,
voestalpine Wire Rod Austria GmbH in St. Peter Freienstein is voestalpine Wire Rod Austria GmbH does not specify a
certified according to EMAS III, ISO 9001, ISO 50001, ISO reference service life for wire rod products. Corrosive
45001 and ISO 14001. As part of the environmental atmospheres must be avoided to guarantee a full lifetime of
declarations required by EMAS, voestalpine Wire Rod Austria functionality.
GmbH continuously publishes environmentally relevant data
and facts about the site. 2.13 Extraordinary effects
Fire
At the St. Peter Freienstein site, investments are constantly Steel wire rod is not flammable, therefore no flammable gases
being made in the expansion of environmental protection or vapours escape.
measures in order to be able to reduce emissions to air and
water to a minimum. Water
No negative consequences for the environment are to be
All operating facilities that have been approved in accordance expected under the influence of water.
with the environmental impact assessment procedure are also
periodically inspected by the authorities as part of Mechanical destruction
environmental inspections. Unpredictable mechanical impact on the declared products has
no negative consequences on the environment due to the
2.8 Product processing/Installation plastic deformability of steel.
Wire Rod products from voestalpine Wire Rod Austria GmbH
are processed by a broad range of different customers in the 2.14 Re-use phase
respective factories. Depending on the desired application, the The declared products from voestalpine Wire Rod Austria
wire rod is further processed in different ways, e.g. drawing, GmbH consist of almost 100 % steel and can therefore be
cold heading, turning, bending or spring coiling. reused or recycled in the steel industry as a secondary raw
material for an unlimited number of circles.
2.9 Packaging
Wire rod is mostly delivered by truck or train. For selected 2.15 Disposal
customers voestalpine Wire Rod Austria is also able to supply The declared product can be fully used as a recycling raw
by ship. material. The waste code according to the European Waste
Catalogue is: 17 04 05 (iron and steel). The waste type is
The products are delivered in coil shape either as a single equivalent to the key number 35103 according to the nationally
bundle (3 t coil) or double bundle (2 x 1,5 t coils). These applicable Waste Catalogue by-law.
bundles are strapped together using metal straps to ensure a
2.16 Further information
stable position on the trucks/train.
Further information on the product is available on the website at
In case the coils are loaded on a ship a seaproof packaging is https://www.voestalpine.com/wiretechnology/en/contact/production-
applied on the wire rod by wrapping it in plastic foil. ites/voestalpine-wire-rod-austria/
3. LCA: Calculation rules
Name Value Unit
3.1 Declared Unit
Declared unit 1 t
This environmental product declaration refers to a declared unit
of 1 tonne of average annealed wire rod.
Density 7850 kg/m3
Declared unit For the calculation of the declared average, input and
production quantities for the entire calendar year 2018 were
3 Environmental Product Declaration - voestalpine Wire Rod Austria GmbH - Annealed wire rod
taken into account and broken down to the declared product assumptions from average data (when available) or with
group. The calculated results can thus be considered generic data and are documented accordingly. Only data with a
representative for the declared product portfolio of annealed contribution of less than 1 % were cut off. Ignoring such data is
wire rod of voestalpine Wire Rod Austria GmbH. justified based on the irrelevance of the expected effect.
Processes, materials, or emissions known to make a significant
A linear correlation of the environmental impacts with the contribution to the environmental effects of the products under
product weight is to be expected. Therefore, the conversion examination have not been neglected. All relevant data were
from the declared unit to a specific product is possible using a collected comprehensively. It is assumed that the data have
mass-specific scaling factor. been completely recorded and the overall total of ignored input
flows do not amount to more than 5 % of total energy and mass
3.2 System boundary flows.
The life cycle assessment of average annealed wire rod refers Environmental impacts of machines, plant and infrastructure
to a cradle-to-gate analysis with modules (A1–A3 + C +D). were not included.
Subsequent life cycle phases are part of the analysis:
3.5 Background data
Module A1–A3 | Production stage This study uses generic background data for the evaluation of
The production stage includes the burdens of the production of upstream environmental impacts from GaBi-database 2021.1
annealed wire rod of voestalpine Wire Rod Austria GmbH at the and is modelled in GaBi-software version 10.
production site in St. Peter Freienstein. The used steel billets
are provided by the integrated steel mill at the production site in 3.6 Data quality
Donawitz. Thus, the upstream environmental impact of the steel The foreground data collected at voestalpine Wire Rod Austria
supplied is represented by primary data of the respective GmbH are based on the quantities used and volumes produced
production site. Material and energy flows for the rolling line, annually. Process data were collected by voestalpine in the
pickling and annealing are considered. Electricity at St. Peter course of reporting to official agencies. Data on material and
Freienstein is provided from the network of the integrated steel energy use originate from material-specific throughput
mill at the production site in Donawitz. The power plant is measurements of various processes as well as from controlling.
represented based on the site-specific conditions. Data for the The technological, geographical and time-related
representation of the power plant refers to the year 2017. Since representativeness of the data base was kept in mind when
2020, Donawitz purchases 100 % green electricity, which is selecting background data. Whenever specific data were
also considered in this EPD. Thermal energy provision is based missing, either generic datasets or representative average data
on natural gas. Module A1–A3 also includes the production of were used instead. The implemented GaBi background
the packaging. datasets are not more than ten years old.
3.7 Period under review
Module C1 | Deconstruction and demolition
It is assumed that the product is not connected with other Foreground data were collected in the 2018 production year,
materials and can therefore be dismantled. Associated efforts and the data are based on the volumes produced on an annual
are negligible, no environmental impacts from the basis.
deconstruction of the products are declared.
3.8 Geographic Representativeness
Land or region, in which the declared product system is
Module C2 | Transport
manufactured, used or handled at the end of the product´s
The transport to the disposal of the material is estimated
lifespan: Austria
declaring a 50 km radius to the waste processing.
Module C3 | Waste processing
Product flows that reach Module D for recycling leave the 3.9 Allocation
product system in C3. Environmental impacts resulting from the
The primary data for the upstream production of the steel billets
grinding and sorting of steel scrap are not included due to the
were allocated using the partitioning approach developed by
negligible expected environmental impact.
worldsteel 2014 for calculating life cycle inventories of co-
products in steel production, which is in line with the provisions
Module C4 | Landfilling
of EN 15804. The so-called partitioning approach provides for
Module C4 declares the environmental impacts incurred by
the allocation of environmental effects on the steelmaking
landfilling (5 % of the product).
process and the emerging byproducts based on physical
relations. Material-inherent flow properties are, thus, taken into
Module D | Benefits and loads beyond the system
account.
boundary
The potential for substituting primary steel with a recycling
Economic allocation is not considered as referring byproducts
scenario (95 % of the product) is outlined in Module D.
and co-products are not directly tradable goods. Furthermore,
long-term contracts for the sale of the byproducts exist, and the
3.3 Estimates and assumptions
negotiated prices are, therefore, not subject to market
All assumptions are verified through detailed documentation
dynamics.
and correspond to the best possible representation of reality
based on the available data. Regional applicability of the used 3.10 Comparability
background data refers to average data under European or
Basically, a comparison or an evaluation of EPD data is only
German conditions taken from the GaBi-database. German
possible if all the data sets to be compared were created
data were used for the Austrian market whenever European or
according to EN 15804 and the building context, respectively
Austrian average data were not available.
the product-specific characteristics of performance, are taken
into account. The GaBi background database was used to
3.4 Cut-off criteria
calculate the LCA (GaBi 10; 2021.1).
All inputs and outputs for which data are available are included
in the LCA model. Data gaps are filled with conservative
4 Environmental Product Declaration - voestalpine Wire Rod Austria GmbH - Annealed wire rod
4. LCA: Scenarios and additional technical information
published in ökobaudat 2022:
Characteristic product properties of biogenic carbon
End of life (C1–C4)
The declared product does not contain any biogenic carbon.
The considered packaging does not contain any biogenic Name Value Unit
carbon either. Collected separately (steel) 1000 kg
Recycling 95 % 950 kg
Landfilling 5 % 50 kg
Installation into the building (A5) Reuse, recovery and/or recycling potentials (D), relevant
scenario information
The end-of-life of the packaging materials is not declared in
Module A5. Name Value Unit
Name Value Unit Net flow of steel scrap 908 kg
Packaging (steel coil) 5.42 kg This scenario contains a recycling rate of 95 %. Since
voestalpine externally purchases scrap for steel production, this
The end-of-life scenario used in this LCA study is based on the
is offset against the steel scrap for recycling (net flow).
following assumptions and thus complies with the specifications
5 Environmental Product Declaration - voestalpine Wire Rod Austria GmbH - Annealed wire rod
5. LCA: Results
The following table contains the LCA results for a declared unit of 1 tonne of annealed wire rod.
DESCRIPTION OF THE SYSTEM BOUNDARY (X = INCLUDED IN LCA; ND = MODULE OR INDICATOR NOT DECLARED; MNR =
MODULE NOT RELEVANT)
Benefits and
Construction loads beyond
Product stage Use stage End of life stage
process stage the system
boundaries
la ire ta m w a Ry lp p u s tro p s n a rT g n iru tc a fu n a M e h t m o rf tro p s n a rTe tis e h t o t e ta g y lb m e s s A e s U e c n a n e tn ia M ria p e R tn e m e c a lp e R tn e m h s ib ru fe R y g re n e la n o ita re p Oe s u re ta w la n o ita re p Oe s u n o itc u rts n o c -e Dn o itilo m e d tro p s n a rT g n is s e c o rp e ts a W la s o p s iD -e s u e R-y re v o c e R-g n ilc y c e Rla itn e to p
A1 A2 A3 A4 A5 B1 B2 B3 B4 B5 B6 B7 C1 C2 C3 C4 D
X X X MND MND MND MND MNR MNR MNR MND MND X X X X X
RESULTS OF THE LCA - ENVIRONMENTAL IMPACT according to EN 15804+A2: 1 tonne annealed wire rod
Parameter Unit A1-A3 C1 C2 C3 C4 D
Global Warming Potential total (GWP-total) kg CO 2 eq 2.95E+03 0 3.02E+00 0 2.42E+00 -1.54E+03
Global Warming Potential fossil fuels (GWP-fossil) kg CO 2 eq 2.93E+03 0 3E+00 0 2.44E+00 -1.54E+03
Global Warming Potential biogenic (GWP-biogenic) kg CO 2 eq 1.66E+01 0 -3.56E-03 0 -2.5E-02 -9.97E-01
Global Warming Potential luluc (GWP-luluc) kg CO 2 eq 9.95E-01 0 2.44E-02 0 2.44E-03 2.23E-01
Depletion potential of the stratospheric ozone layer (ODP) kg CFC11 eq 8.21E-12 0 5.9E-16 0 5.77E-15 -2.57E-12
Acidification potential of land and water (AP) mol H+ eq 9.16E+00 0 9.92E-03 0 7.78E-03 -2.76E+00
Eutrophication potential aquatic freshwater (EP-freshwater) kg P eq 1.07E-02 0 8.88E-06 0 1.86E-06 -3.15E-04
Eutrophication potential aquatic marine (EP-marine) kg N eq 2.21E+00 0 4.55E-03 0 1.93E-03 -4.12E-01
Eutrophication potential terrestrial (EP-terrestrial) mol N eq 2.38E+01 0 5.08E-02 0 2.12E-02 -4.01E+00
Formation potential of tropospheric ozone photochemical oxidants kg NMVOC
7.5E+00 0 8.94E-03 0 6.08E-03 -2.11E+00
(POCP) eq
Abiotic depletion potential for non fossil resources (ADPE) kg Sb eq 5.2E-03 0 2.65E-07 0 1.68E-07 -3.35E-03
Abiotic depletion potential for fossil resources (ADPF) MJ 2.66E+04 0 3.98E+01 0 3.56E+01 -1.34E+04
m3 world eq
Water use (WDP) 2.82E+02 0 2.77E-02 0 -2.89E-02 -3.02E+02
deprived
RESULTS OF THE LCA - INDICATORS TO DESCRIBE RESOURCE USE according to EN 15804+A2: 1 tonne annealed wire rod
Parameter Unit A1-A3 C1 C2 C3 C4 D
Renewable primary energy as energy carrier (PERE) MJ 1.98E+03 0 2.29E+00 0 2.57E+00 1.23E+03
Renewable primary energy resources as material utilization
MJ 0 0 0 0 0 0
(PERM)
Total use of renewable primary energy resources (PERT) MJ 1.98E+03 0 2.29E+00 0 2.57E+00 1.23E+03
Non renewable primary energy as energy carrier (PENRE) MJ 2.67E+04 0 4E+01 0 3.56E+01 -1.34E+04
Non renewable primary energy as material utilization (PENRM) MJ 0 0 0 0 0 0
Total use of non renewable primary energy resources (PENRT) MJ 2.67E+04 0 4E+01 0 3.56E+01 -1.34E+04
Use of secondary material (SM) kg 9.16E+01 0 0 0 0 9.08E+02
Use of renewable secondary fuels (RSF) MJ 0 0 0 0 0 0
Use of non renewable secondary fuels (NRSF) MJ 0 0 0 0 0 0
Use of net fresh water (FW) m3 1.53E+01 0 2.62E-03 0 3.67E-04 -6.78E+00
RESULTS OF THE LCA – WASTE CATEGORIES AND OUTPUT FLOWS according to EN 15804+A2:
1 tonne annealed wire rod
Parameter Unit A1-A3 C1 C2 C3 C4 D
Hazardous waste disposed (HWD) kg 5.59E-06 0 2.11E-09 0 6.3E-09 3.74E-06
Non hazardous waste disposed (NHWD) kg 3.92E+01 0 6.27E-03 0 5.01E+01 1.61E+02
Radioactive waste disposed (RWD) kg 2.4E-01 0 7.25E-05 0 4.05E-04 4.85E-04
Components for re-use (CRU) kg 0 0 0 0 0 0
Materials for recycling (MFR) kg 0 0 0 9.5E+02 0 0
Materials for energy recovery (MER) kg 0 0 0 0 0 0
Exported electrical energy (EEE) MJ 0 0 0 0 0 0
Exported thermal energy (EET) MJ 0 0 0 0 0 0
RESULTS OF THE LCA – additional impact categories according to EN 15804+A2-optional:
1 tonne annealed wire rod
Parameter Unit A1-A3 C1 C2 C3 C4 D
Disease
Incidence of disease due to PM emissions (PM) ND ND ND ND ND ND
incidence
Human exposure efficiency relative to U235 (IR) kBq U235 eq ND ND ND ND ND ND
Comparative toxic unit for ecosystems (ETP-fw) CTUe ND ND ND ND ND ND
Comparative toxic unit for humans (carcinogenic) (HTP-c) CTUh ND ND ND ND ND ND
6 Environmental Product Declaration - voestalpine Wire Rod Austria GmbH - Annealed wire rod
Comparative toxic unit for humans (noncarcinogenic) (HTP-nc) CTUh ND ND ND ND ND ND
Soil quality index (SQP) SQP ND ND ND ND ND ND
The additional and optional impact categories according to EN 15804+A2 are not declared, as the uncertainty of these indicators is to
be classified as high.
Disclaimer 1 – for the indicator potential human exposure efficiency relative to U235:
This impact category deals mainly with the eventual impact of low dose ionizing radiation on human health of the nuclear fuel cycle. It
does not consider effects due to possible nuclear accidents, occupational exposure nor radioactive waste disposal in underground
facilities. Potential ionizing radiation from the soil, from radon and from some construction materials is also not measured by this
indicator.
Disclaimer 2 – for the indicators abiotic depletion potential for non-fossil resources,abiotic depletion potential for fossil resources, water
(user) deprivation potential, deprivation weighted water consumption, eutrophication fraction of nutrients reaching freshwater end
compartment, potential comparative toxic unit for humans cancerogenic, potential comparative toxic unit for humans not cancerogenic,
potential soil quality index:
The results of this environmental impact indicator shall be used with care as the uncertainties on these results are high or as there is
limited experience with the indicator.
6. LCA: Interpretation
The following interpretation contains a summary of the LCA wire rod.
results referenced to a declared unit of 1 tonne of annealed
A comparison of the individual lifecycle phases results in a clear
dominance of the production phase (modules A1–A3). The Most of the potential environmental impacts of the production
environmental effects in the production phase are mainly phase (module A1–A3) of the annealed wire rod can be traced
dominated by the direct process emissions of billet production. back to the billet production in Donawitz. The production of
annealed wire rod at the production site at St. Peter Freienstein
As a result of product recyclability, the material removed at the contributes app. 10 % to global warming potential.
end of life can substitute primary steel. According to the set
method, the first step is to saturate the secondary material used A linear correlation of the environmental impacts with the
in module A with material from module C. The excess amount product weight is to be expected. Therefore, the conversion
from module C ('net flow') can substitute primary steel and from the declared unit to a specific product is possible using a
leads to corresponding substitution potentials in module D. mass-specific scaling factor.
The environmental impact of the transport of the products to All primary data were specifically broken down to the declared
recycling (C2) as well as landfilling of the losses at the end of product group. As a result, the representativity of the results for
life (C4) represents a minor contribution to the overall the declared product group is to be expected as high.
environmental impact of the product.
7 Environmental Product Declaration - voestalpine Wire Rod Austria GmbH - Annealed wire rod
7. Requisite evidence
Not relevant for this EPD.
8. References
Standards 761/2001 and Commission Decisions 2001/681/EC and
2006/193/EC.
EN 10027-1
DIN EN 10027-1:2016, Designation systems for steels - Part 1: European Waste Catalogue
Steel names. Guidance on classification of waste according to EWC Stat
categories. Supplement to the Manual for the Implementation of
EN 10108 the Regulation (EC) No 2150/2002 on Waste Statistics.
DIN EN 10108:2004, Round steel rod for cold heading and cold Commission of the European Communities, EUROSTAT.
extrusion Dimensions and tolerances.
GaBi
EN 15804 GaBi 10, Software System and Database for Life Cycle
DIN EN 15804:2012+A2:2019+AC:2021, Sustainability of Engineering. DB 2021.1. Sphera, 1992-2021. Available in:
construction works - Environmental product declarations - Core http://documentation.gabisoftware.com
rules for the product category of construction products.
IBU 2021
ISO 9001 Institut Bauen und Umwelt e.V.: General guidance for the EPD
DIN EN ISO 9001:2015-11, Quality management systems - program of the Institut Bauen und Umwelt e.V.. (IBU). Version
Requirements. 2.0, Berlin: Institut Bauen und Umwelt e.V., 2021.
www.ibu-epd.com
ISO 14001
DIN EN ISO 14001:2015-11, Environmental management Key to Steel
systems - requirements with guidance for use. Key to Steel (Stahlschlüssel) 2019, 25. edition, 2023, Verlag
Stahlschlüssel Wegst GmbH, Germany.
ISO 14025
DIN EN ISO 14025:2011-10, Environmental labels and ökobaudat 2022
declarations - Type III environmental ökobaudat 2022. EN 15804 and BNB compliant data for over
declarations - Principles and procedures. 700 building products.
ISO 14044 Ordinance on Biocide Products
DIN EN ISO 14044:2006-10, Environmental management - Life Regulation (EU) No 528/2012 of the European Parliament and
cycle assessment - Requirements and guidance. of the Council of 22 May 2012 concerning the making available
on the market and use of biocidal products.
ISO 45001
DIN EN ISO 45001:2018-03, Occupational health and safety PCR Part A
management systems - Requirements with guidance for use. Product category rules for building-related products and
services. Part A: Calculation rules for life cycle assessment and
ISO 50001 project report requirements according to EN 15804+A2:2019.
DIN EN ISO 50001:2018-12, Energy management systems - Version 1.3. Berlin: Institut Bauen und Umwelt e.V.. (ed.), 2022.
Requirements with guidance for use.
PCR: Structural steels
Further references Product category rules for building-related products and
services. Part B: Requirements for the EPD for structural steels.
Candidate list Version v0. Berlin: Institut Bauen und Umwelt e.V., 08.03.2023.
Candidate List of Substances of Very High Concern (ECHA
Candidate List) of 16.01.2020, published in accordance with worldsteel 2014
Article 59 (10) of the REACH Regulation Helsinki: European World Steel Association, February 14, 2014: A methodology to
Chemicals Agency. determine the LCI of steel industry co-products.
EMAS III worldsteel 2019
Regulation (EC) No 1221/2009 of the European parliament and World Steel Association, 2019: Life cycle inventory
of the council of 25 November 2009 on the voluntary methodology report.
participation by organisations in a Community eco-management
and audit scheme (EMAS), repealing Regulation (EC) No
8 Environmental Product Declaration - voestalpine Wire Rod Austria GmbH - Annealed wire rod
Publisher
Institut Bauen und Umwelt e.V. +49 (0)30 3087748- 0
Hegelplatz 1 info@ibu-epd.com
10117 Berlin www.ibu-epd.com
Germany
Programme holder
Institut Bauen und Umwelt e.V. +49 (0)30 3087748- 0
Hegelplatz 1 info@ibu-epd.com
10117 Berlin www.ibu-epd.com
Germany
Author of the Life Cycle Assessment
Daxner & Merl GmbH +43 676 849477826
Schleifmühlgasse 13/24 office@daxner-merl.com
1040 Wien www.daxner-merl.com
Austria
Owner of the Declaration
voestalpine AG +43/50304/15-0
voestalpine-Straße 3 info@voestalpine.com
4020 Linz www.voestalpine.com
Austria
9 Environmental Product Declaration - voestalpine Wire Rod Austria GmbH - Annealed wire rod
