ENVIRONMENTAL PRODUCT DECLARATION
as per ISO 14025 and EN 15804+A2
Owner of the Declaration fischerwerke GmbH & Co. KG
Programme holder Institut Bauen und Umwelt e.V. (IBU)
Publisher Institut Bauen und Umwelt e.V. (IBU)
Declaration number EPD-FIW-20210314-CBD1-EN
Issue date 22.02.2022
Valid to 21.02.2027
Insulation fixings
fischerwerke GmbH & Co. KG
www.ibu-epd.com | https://epd-online.com
Umwelt Produktdeklaration Name des Herstellers – Name des Produkts
General Information
fischerwerke GmbH & Co. KG Insulation anchors
Programme holder Owner of the declaration
IBU – Institut Bauen und Umwelt e.V. fischerwerke GmbH & Co. KG
Panoramastr. 1 Klaus-Fischer-Straße 1
10178 Berlin 72178 Waldachtal
Germany Germany
Declaration number Declared product / declared unit
EPD-FIW-20210314-CBD1-EN The declaration refers to the production of average
ETICS anchors for fastening 1 square meter (sq m)
ETICS system with the usable lengths 75 - 120 mm,
121 - 140 mm and 141 - 160 mm. The core EPD
contains the data and results for the usable lengths
121 - 140 mm. The additional usable lengths are
declared in the annexe. 5 anchors per sq m ETICS
system are required. The average is calculated
depending on the produced annual quantity of the
products mentioned under chapter “Product
description/Product definition”.
This declaration is based on the product Scope:
category rules: This EPD refers to average ETICS anchors
Wall plugs made of plastic and metal, 11.2017 manufactured at the plant in Waldachtal Germany and
(PCR checked and approved by the SVR) at fischer Vyskov spol s.r.o in Ivanovice na Hané in the
Czech Republic. The data basis is the year 2020.
Issue date
22.02.2022 The owner of the declaration shall be liable for the
underlying information and evidence; the IBU shall not
be liable with respect to manufacturer information, life
Valid to
cycle assessment data and evidences.
21.02.2027
The EPD was created according to the specifications
of EN 15804+A2. In the following, the standard will be
simplified as EN 15804.
Verification
The standard EN 15804 serves as the core PCR
Independent verification of the declaration and data
according to ISO 14025:2010
Dipl. Ing. Hans Peters internally x externally
(chairman of Institut Bauen und Umwelt e.V.)
Dr. Alexander Röder Prof. Dr. Birgit Grahl
(Managing Director Institut Bauen und Umwelt e.V.)) (Independent verifier)
Product
Information about the enterprise from the following product range are considered. The
fischerwerke GmbH & Co. KG is certified according to following system-related and non-system-related
ISO 9001 quality management systems, ISO 14001 insulation anchors (product names) are preferably
environmental management systems (DQS GmbH used in ETICS facades (external thermal insulation
under certificate registration no. 393802 UM). composite system):
 TermoZ PN, CN, CNplus, CS 8, CS II,
Product description/Product definition CS 8 DT 110 V, CS II DT 110 V , 8U, SV II
Fixing systems from fischerwerke GmbH & Co. KG are
with accessories.
made of different materials. These consist of a sleeve
 TermoZ 6H
made of plastic and an expansion element made of
steel or plastic and be delivered in recyclable cartons.  TermoFix 6H-NT, B, H
All product components consist of new and recycled  Additional plate DT 90, DT 110, DT 140
materials. The anchors differ, for example, in their  FIF-PN, FIF-CN, FIF-CS, FIF-SV II, DIPK
specific effective length. The declaration applies to
average anchors used in 3 different external thermal
insulation composite systems (ETICS) with different
effective lengths. For the averaging, insulation anchors
2 Environmental Product Declaration fischerwerke GmbH & Co. KG – Insulation fixings
The following insulation anchors are preferably used in the relevant technical provision (no CE-marking) or
VHF façades (curtain-type, rear-ventilated façade): with respect to its technical data sheets.
 DHK The main technical parameters for usable length 121-
 DHM, FDM 140mm are listed in the following table.
Name Value Unit
The anchors are used for ETICS include the following Screw diameter 4.4 - 6 mm
usable lengths: Wall plug diameter 8 - 10 mm
 75 - 120 mm Plate diameter 45 - 110 mm
 121 - 140 mm Drill hole depth 35 - 90 mm
 141 - 160 mm Anchoring depth 25 - 80 mm
Plate stiffness of the anchor acc.
0.6 - 1.29 kN/mm
EOTA Technical Report TR 026
fischer anchors with a working length of more than 160
Spot-related heat transition
mm are covered in the EPD "ETICS Anchors" of the
coefficient (Chi value) of the
VDPM (Verband für Dämmsysteme, Putz und Mörtel 0 - 0.002 W/K
anchor acc. EOTA Technical
e.V.). The results are shown for the usable length 121 -
Report TR 025
140 mm. The results for the other usable lengths (75 -
120 mm and 141 - 160 mm) are presented in the
annexe.
The product portfolio includes products which have a
Base materials/Ancillary materials
European Technical Assessment or national approval
by the building authorities, as well as products without
The basic materials or pre-products for fischer
any approval. For further information see
insulation anchors and their mass-related share of the
www.fischer-international.com
total product are listed in the following chart:
For the placing of the product on the market in the
Name Value Unit
European Union/European Free Trade Association
Polyamide PA 6 7 %
/EU/EFTA) the Regulation (EU) No. 305/2011 (CPR)
Polyamide PA 6 glass fibre
applies. The product needs a declaration of 36 %
reinforced
performance taking into consideration of an ETA on
Polyethylene PE-HD 0 %
the basis of the guideline EOTA EAD 330196-01-0604
Polypropylene PP 14 %
or EOTA ETAG 014 and the CE-marking.
The rules of application are regulated in EOTA ETAG Steel 42 %
014 or EOTA EAD 330196-01-0604. Situationally, the EPS 0.1 %
respective national regulations also apply.
1) This product/article/at least one partial article
The use of products with national approvals is subject contains substances listed in the candidate list (date:
to the respective national regulations at the place of 17.12.2021) exceeding 0.1 percentage by mass:
use apply and the technical regulations based on these no.
regulations.
2) This product/article/at least one partial article
Application contains other carcinogenic, mutagenic, reprotoxic
The anchors used in ETICS are installed in a push- (CMR) substances in categories 1A or 1B which are
through installation. In this process, the same drill not on the candidate list, exceeding 0.1 percentage by
diameter is drilled through the installation object mass: no.
(insulation material or support rail) as in the substrate.
The anchor is then pushed through the installation 3) Biocide products were added to this construction
object into the drill hole and expanded. There is no product or it has been treated with biocide products
impact on the environment and health after correct use (this then concerns a treated product as defined by the
(usage). Approved insulation anchors cannot be re- (EU) Ordinance on Biocide Products No. 528/2012:
used due to the approval. no.
For ETICS anchors, the maximum useful length is
specified by the anchor. To determine the required In addition to the raw material, auxiliary and operating
effective length, the product declaration fischerwerke materials are used for processing and finishing. These
GmbH & Co. KG - Insulation anchor, thickness of the auxiliary and operating materials are subject to
insulation material, the adhesive layer and any existing continuous monitoring. If they can no longer be used,
non-load-bearing layers (old plaster, insulation, etc.) they are recycled externally by specialised waste
must be taken into account. When fixing through the management companies.
mesh, the thickness of the base plaster must be taken
into account. Reference service life
The lifetime of the insulation anchors is verified
Technical Data according to EOTA EAD 040083-00-0404. This
Performance data of the product in accordance with assumes a lifetime for the ETICS of at least 25 years.
the declaration of performance with respect to its
essential characteristics according to its specific ETA
or with respect to its characteristics in accordance with
3 Environmental Product Declaration fischerwerke GmbH & Co. KG – Insulation fixings
LCA: Calculation rules
Declared Unit System boundary
This declaration refers to the declared unit of 1m2 The type of EPD is cradle to factory gate - with options.
average ETICS system with a specific usable length, The environmental product declaration relates to the
given in mm. The average dowels used for ETICS production stage (module A1: provision of raw
systems with 3 different usable lengths (75 - 120 mm; materials; A2: transport; A3: manufacture). The
121 - 140 mm; 141 - 160 mm) are calculated. The energetic recovery of the packaging (A5), reuse,
usable length of 121 - 140 mm is declared in the EPD recovery (C3) as well as the dumping of the dowels
and the 2 other usable lengths are in the annexe. (C4) including credits outside the system boundary
“Average” describes all the anchor types produced in a (module D) are taken into account. The product
specific usable length class. The average is calculated installation (module A4) as well as the usage stage
according to production shares (quantities). The (module B) and the dismantling / demolition (C1) are
dowels were grouped according to their useful lengths. not taken into account in this study. Transport of the
The quality of the relevant data used for the EPD in waste to the landfill (100 km) is taken into account (C2)
terms of its time, geography and technology The waste is treated further (C3) and a closed-loop
representativeness is mostly very good. scenario has been modelled in the end-of-life (EoL)
The current average number of anchors is 5 anchors phase.
per m2 (as used in the EPD ETICS). In order to be able The dowels produced in Germany and the Czech
to convert the declared unit of 1 m2 average ETICS Republic are modelled on the boundary conditions
system to one kg dowel, it must be multiplied by the typical for each country (electricity, diesel). The
required conversion factor. To get the results for 1 material composition and the energy requirement of
dowel, the results have to be divided by 5. the average dowels were calculated according to their
production shares (based on the quantity) in the two
Specification of the declared unit production countries.
Name Value Unit
Conversion factor to 1 kg (mass Comparability
0.1388 -
in kg per declared unit) Basically, a comparison or an evaluation of EPD data
Declared unit 5 Pce/m2 is only possible if all the data sets to be compared
system
were created according to EN 15804 and the building
context, respectively the product-specific
characteristics of performance, are taken into account.
Background database: GaBi ts software, CUP 2020.2.
LCA: Scenarios and additional technical information
Characteristic product properties landfilled. A transport distance of 100 km to the landfill
Information on biogenic Carbon is assumed.
Information on describing the biogenic Carbon Reuse, recovery and recycling potential (D)
Content at factory gate Module D considers the credit from the three end-of-
Name Value Unit life scenarios. D/1 represents the credit related to the
Biogenic Carbon Content in incineration of plastic and recycling benefits of steel
0.66 kg C
accompanying packaging considered in the incineration scenario. D/2 represents
the credit linked to the incineration of packaging
material considered in module A5 in the landfill
The following technical scenario information is required scenario whereas the D/3 represents the material
for the declared modules. credit along with incineration of plastic considered in a
closed-loop scenario.
Installation in the building (A5)
Name Value Unit
Output substances following
waste treatment on site 3.1E-06 kg
(packaging material)
End of Life (C1-C4)
Name Value Unit
Collected separately waste type 0.1388 kg
There are three scenarios for 100% of the used
product that have been considered. C3/1 represents
the generic incineration scenario and C3/2 represents
the incineration considered in the close loop Scenario
in EoL phase. In C4 the product is completely
4 Environmental Product Declaration fischerwerke GmbH & Co. KG – Insulation fixings
LCA: Results
Disclaimer EP-freshwater:
This indicator has been calculated as “kg P eq” as required in the characterisation model (EUTREND model,
Struijs et al., 2009b, as implemented in ReCiPe; http://eplca.jrc.ec.europa.eu/LCDN/developerEF.xhtml).
DESCRIPTION OF THE SYSTEM BOUNDARY (X = INCLUDED IN LCA; ND = MODULE OR INDICATOR NOT
DECLARED; MNR = MODULE NOT RELEVANT)
BENEFITS AND
CONSTRUCTI LOADS
PRODUCT STAGE ON PROCESS USE STAGE END OF LIFE STAGE BEYOND THE
STAGE SYSTEM
BOUNDARIES
5 Environmental Product Declaration fischerwerke GmbH & Co. KG – Insulation fixings
lairetam
waR
ylppus tropsnarT
gnirutcafunaM
eht
morf
tropsnarT
etis
eht
ot
etag
ylbmessA esU
ecnanetniaM
riapeR
tnemecalpeR tnemhsibrufeR
ygrene
lanoitarepO esu
retaw
lanoitarepO esu
noitcurtsnoc-eD
noitilomed tropsnarT
gnissecorp
etsaW
lasopsiD -esueR -yrevoceR -gnilcyceR laitnetop
A1 A2 A3 A4 A5 B1 B2 B3 B4 B5 B6 B7 C1 C2 C3 C4 D
X X X ND X ND ND MNR MNR MNR ND ND X X X X X
RESULTS OF THE LCA - ENVIRONMENTAL IMPACT according to EN 15804+A2: 1 m² ETICS system (121-
140mm)
Core Indicator Unit A1-A3 A5 C1 C2 C3/1 C3/2 C4 D/1 D/2 D/3
GWP-total [kg CO2-Eq.] 7.15E-1 1.15E-2 0.00E+0 1.16E-3 1.60E-1 1.29E-2 7.81E-3 -2.12E-1 -4.60E-3 -6.97E-1
GWP-fossil [kg CO2-Eq.] 7.26E-1 9.30E-4 0.00E+0 1.15E-3 1.60E-1 1.29E-2 8.07E-3 -2.11E-1 -4.57E-3 -6.95E-1
GWP-biogenic [kg CO2-Eq.] -1.13E-2 1.05E-2 0.00E+0 -1.97E-6 7.88E-6 1.29E-5 -2.71E-4 -8.70E-5 -1.92E-5 -2.43E-3
GWP-luluc [kg CO2-Eq.] 5.00E-4 8.06E-7 0.00E+0 9.32E-6 3.59E-6 5.61E-6 7.64E-6 -5.10E-5 -5.92E-6 -1.77E-4
ODP [kg CFC11-Eq.] 9.70E-14 3.50E-18 0.00E+0 1.38E-19 3.67E-17 8.42E-17 1.91E-17 -1.23E-16 -7.09E-17 -1.84E-15
AP [mol H+-Eq.] 1.38E-3 3.94E-6 0.00E+0 4.04E-6 4.75E-5 1.09E-5 2.66E-5 -4.71E-4 -5.05E-6 -8.32E-4
EP-freshwater [kg PO4-Eq.] 1.25E-6 8.58E-10 0.00E+0 3.50E-9 6.43E-9 1.03E-8 1.38E-6 -1.13E-7 -9.69E-9 -5.53E-7
EP-marine [kg N-Eq.] 3.59E-4 1.37E-6 0.00E+0 1.85E-6 1.46E-5 2.66E-6 6.04E-6 -1.05E-4 -1.63E-6 -2.72E-4
EP-terrestrial [mol N-Eq.] 3.54E-3 1.84E-5 0.00E+0 2.06E-5 2.26E-4 3.21E-5 6.62E-5 -1.13E-3 -1.74E-5 -2.44E-3
POCP [kg NMVOC-Eq.] 1.03E-3 3.45E-6 0.00E+0 3.59E-6 3.82E-5 7.19E-6 1.94E-5 -3.38E-4 -4.38E-6 -7.50E-4
ADPE [kg Sb-Eq.] 1.27E-5 5.87E-11 0.00E+0 8.25E-11 5.21E-10 1.11E-9 5.57E-10 -8.82E-9 -9.99E-10 -7.53E-8
ADPF [MJ] 1.12E+1 5.27E-3 0.00E+0 1.53E-2 4.18E-2 6.80E-2 1.15E-1 -2.28E+0 -6.55E-2 -1.34E+1
[m³ world-Eq
WDP 2.25E-4 1.37E-3 0.00E+0 1.03E-5 1.63E-2 1.74E-3 -2.94E-5 -4.03E-3 -5.27E-5 1.44E-2
deprived]
GWP = Global warming potential; ODP = Depletion potential of the stratospheric ozone layer; AP = Acidification potential of land and water; EP =
Caption Eutrophication potential; POCP = Formation potential of tropospheric ozone photochemical oxidants; ADPE = Abiotic depletion potential for non-
fossil resources; ADPF = Abiotic depletion potential for fossil resources; WDP = Water (user) deprivation potential
RESULTS OF THE LCA - INDICATORS TO DESCRIBE RESOURCE USE according to EN 15804+A2: 1 m²
ETICS system (121-140mm)
Indicator Unit A1-A3 A5 C1 C2 C3/1 C3/2 C4 D/1 D/2 D/3
PERE [MJ] 1.17E+0 2.68E-2 0.00E+0 8.61E-4 8.68E-3 2.96E-2 8.51E-3 -1.37E-1 -1.66E-2 -4.41E-1
PERM [MJ] 2.59E-2 -2.59E-2 0.00E+0 0.00E+0 0.00E+0 0.00E+0 0.00E+0 0.00E+0 0.00E+0 0.00E+0
PERT [MJ] 1.19E+0 9.12E-4 0.00E+0 8.61E-4 8.68E-3 2.96E-2 8.51E-3 -1.37E-1 -1.66E-2 -4.41E-1
PENRE [MJ] 8.50E+0 6.51E-3 0.00E+0 1.53E-2 2.77E+0 6.80E-2 1.15E-1 -2.29E+0 -6.55E-2 -1.34E+1
PENRM [MJ] 2.73E+0 -1.24E-3 0.00E+0 0.00E+0 -2.73E+0 0.00E+0 0.00E+0 0.00E+0 0.00E+0 0.00E+0
PENRT [MJ] 1.12E+1 5.27E-3 0.00E+0 1.53E-2 4.18E-2 6.80E-2 1.15E-1 -2.29E+0 -6.55E-2 -1.34E+1
SM [kg] 0.00E+0 0.00E+0 0.00E+0 0.00E+0 0.00E+0 0.00E+0 0.00E+0 0.00E+0 0.00E+0 0.00E+0
RSF [MJ] 0.00E+0 0.00E+0 0.00E+0 0.00E+0 0.00E+0 0.00E+0 0.00E+0 0.00E+0 0.00E+0 0.00E+0
NRSF [MJ] 0.00E+0 0.00E+0 0.00E+0 0.00E+0 0.00E+0 0.00E+0 0.00E+0 0.00E+0 0.00E+0 0.00E+0
FW [m³] 1.47E-3 3.24E-5 0.00E+0 9.97E-7 3.85E-4 5.55E-5 3.07E-6 -3.71E-4 -9.07E-6 -1.15E-3
PERE = Use of renewable primary energy excluding renewable primary energy resources used as raw materials; PERM = Use of
renewable primary energy resources used as raw materials; PERT = Total use of renewable primary energy resources; PENRE = Use of
non-renewable primary energy excluding non-renewable primary energy resources used as raw materials; PENRM = Use of non-
Caption
renewable primary energy resources used as raw materials; PENRT = Total use of non-renewable primary energy resources; SM = Use
of secondary material; RSF = Use of renewable secondary fuels; NRSF = Use of non-renewable secondary fuels; FW = Use of net fresh
water
RESULTS OF THE LCA – WASTE CATEGORIES AND OUTPUT FLOWS according to EN 15804+A2:
1 m² ETICS system (121-140mm)
Indicator Unit A1-A3 A5 C1 C2 C3/1 C3/2 C4 D/1 D/2 D/3
HWD [kg] 1.51E-8 6.27E-11 0.00E+0 7.14E-10 7.76E-11 3.16E-11 5.00E-10 -1.37E-9 -3.45E-11 -3.72E-9
NHWD [kg] 8.13E-3 2.30E-4 0.00E+0 2.35E-6 3.39E-3 2.40E-4 1.39E-1 -2.47E-3 -3.11E-5 -3.14E-3
RWD [kg] 1.87E-4 1.22E-7 0.00E+0 1.90E-8 1.25E-6 1.00E-5 1.38E-6 -6.44E-5 -2.41E-6 -6.54E-5
CRU [kg] 0.00E+0 0.00E+0 0.00E+0 0.00E+0 0.00E+0 0.00E+0 0.00E+0 0.00E+0 0.00E+0 0.00E+0
MFR [kg] 0.00E+0 0.00E+0 0.00E+0 0.00E+0 6.94E-2 0.00E+0 0.00E+0 0.00E+0 0.00E+0 0.00E+0
MER [kg] 0.00E+0 0.00E+0 0.00E+0 0.00E+0 0.00E+0 0.00E+0 0.00E+0 0.00E+0 0.00E+0 0.00E+0
EEE [MJ] 0.00E+0 1.46E-2 0.00E+0 0.00E+0 2.68E-1 1.53E-2 0.00E+0 0.00E+0 0.00E+0 0.00E+0
EET [MJ] 0.00E+0 3.36E-2 0.00E+0 0.00E+0 6.15E-1 3.50E-2 0.00E+0 0.00E+0 0.00E+0 0.00E+0
HWD = Hazardous waste disposed; NHWD = Non-hazardous waste disposed; RWD = Radioactive waste disposed; CRU = Components
Caption for re-use; MFR = Materials for recycling; MER = Materials for energy recovery; EEE = Exported electrical energy; EEE = Exported
thermal energy
RESULTS OF THE LCA – additional impact categories according to EN 15804+A2-optional:
1 m² ETICS system (121-140mm)
Indicator Unit A1-A3 A5 C1 C2 C3/1 C3/2 C4 D/1 D/2 D/3
[Disease
PM 1.20E-8 2.25E-11 0.00E+0 2.21E-11 2.63E-10 8.40E-11 2.70E-10 -5.72E-9 -3.81E-11 -5.31E-9
Incidence]
[kBq U235-
IR 1.59E-2 1.13E-5 0.00E+0 2.75E-6 1.13E-4 1.64E-3 1.93E-4 -1.17E-2 -2.17E-4 -5.90E-3
Eq.]
ETP-fw [CTUe] 5.45E+0 2.80E-3 0.00E+0 1.08E-2 1.62E-2 2.90E-2 1.10E-1 -4.36E-1 -1.15E-2 -7.42E+0
HTP-c [CTUh] 3.36E-10 1.21E-13 0.00E+0 2.27E-13 1.66E-12 8.69E-13 5.41E-12 -2.28E-10 -6.46E-13 -1.84E-10
HTP-nc [CTUh] 8.00E-9 5.15E-12 0.00E+0 1.35E-11 1.04E-10 3.42E-11 4.50E-10 -1.23E-9 -2.66E-11 -7.68E-9
SQP [-] 2.57E+0 1.62E-3 0.00E+0 5.38E-3 1.16E-2 2.15E-2 9.00E-3 -9.87E-2 -1.47E-2 -3.96E-1
PM = Potential incidence of disease due to PM emissions; IR = Potential Human exposure efficiency relative to U235; ETP-fw = Potential
Caption comparative Toxic Unit for ecosystems; HTP-c = Potential comparative Toxic Unit for humans (cancerogenic); HTP-nc = Potential
comparative Toxic Unit for humans (not cancerogenic); SQP = Potential soil quality index
Disclaimer 1 – for the indicator IRP
This impact category deals mainly with the eventual impact of low dose ionizing radiation on human health of the
nuclear fuel cycle. It does not consider effects due to possible nuclear accidents, occupational exposure nor
radioactive waste disposal in underground facilities. Potential ionizing radiation from the soil, from radon and from
some construction materials is also not measured by this indicator.
Disclaimer 2 – for the indicators ADPE, ADPF, WDP, ETPfw, HTPc, HTPnc, SQP. The results of this
environmental impact indicator shall be used with care as the uncertainties on these results are high or as there is
limited experienced with the indicator.
6 Environmental Product Declaration fischerwerke GmbH & Co. KG – Insulation fixings
References
IBU 2021 EOTA Technical Report TR 025
General Instructions for the EPD programme of Institut Point thermal transmittance of plastic anchors for
Bauen und Umwelt e.V. Version 2.0, Berlin: Institut ETICS, 2016
Bauen und Umwelt e.V., 2021. www.ibu-epd.com
EOTA Technical Report TR 026
PCR Part A Plate stiffness of plastic anchors for ETICS, 2016
PCR - Part A: Calculation Rules for the Life Cycle
Assessment and Requirements on the Project Report, EPD “ETICS Anchors”
Berlin: Institut Bauen und Umwelt e.V., www.ibu- Environmental Product Declaration: WDVS mit EPS
epd.com, 2020 geklebt und gedübelt (ETICS with EPS glued and
anchored), VDPM (Verband für Dämmsysteme, Putz
PCR Part B und Mörtel e.V.), EPD-WDV-20170077-IBG2-DE.
PCR Part B: Requirements on the EPD for Wall plugs Berlin: Institut Bauen und Umwelt e.V. (Ed.), Jun 07,
made of plastic and metal, Berlin: Institut Bauen und 2017.
Umwelt e.V., 11-2017 Environmental Product Declaration: WDVS mit
Mineralfaser Dämmplatte geklebt und gedübelt (ETICS
ISO 4042 with mineral wool insulation board glued and
ISO 4042:2018-08, Fasteners - Electroplated coating anchored), VDPM (Verband für Dämmsysteme, Putz
systems und Mörtel e.V.), EPD-WDV-20170078-IBG2-DE.
Berlin: Institut Bauen und Umwelt e.V. (Ed.), Jun 07,
ISO 9001 2017.
DIN EN ISO 9001:2015-11, Quality management
systems - Requirements (ISO 9001:2015) ETA
European Technical Assessment (e.g. ETA-14/0372
ISO 14001 for TermoZ plastic anchors), 2021
DIN EN ISO 14001:2015-11, Environmental
management systems - Requirements with guidance GaBi ts software
for use Sphera Solutions GmbH
GaBi Software System and Database for Life Cycle
ISO 14025 Engineering
DIN EN ISO 14025:2011-10, Environmental labels and CUP Version: 2020.2
declarations — Type III environmental declarations — University of Stuttgart
Principles and procedures LeinfeldenEchterdingen
EN 15804 GaBi ts documentation
EN 15804:2019+A2, Sustainability of construction GaBi life cycle inventory data documentation
works — Environmental Product Declarations — Core (https://www.gabisoftware.
rules for the product category of construction products. com/support/gabi/gabidatabase2020lcidocumentation/)
CPR Ordinance on Biocide Products
REGULATION (EU) No 305/2011 OF THE REGULATION (EU) No 528/2012 OF THE
EUROPEAN PARLIAMENT AND OF THE COUNCIL EUROPEAN PARLIAMENT AND OF THE COUNCIL
of 9 March 2011 laying down harmonised conditions of 22 May 2012 concerning the making available on
for the marketing of construction products and the market and use of biocidal products,
repealing Council Directive 89/106/EEC, Official Ordinance regulating the manufacture, labelling,
Journal of the European Union, 2011 placing on the market and use of biocidal products.
Official Journal of the European Union, 2012
EOTA ETAG 014
Guideline for European Technical Approval of plastic REACH/ECHA candidate list
anchors for fixing of external thermal insulation List of substances considered for authorisation
composite systems with rendering, 2011 substances of very high concern (SVHCs)
(ECHA candidate list), published in accordance with
EOTA EAD 040083-00-0404 Article 59, paragraph 10 of the REACH, Regulation
European Assessment Document for external thermal Helsinki: European Chemicals Agency, view of
insulation composite systems (ETICS) with renderings, 17.12.2021
2019
Technical data sheets of engineered products,
EOTA EAD 330196-01-0604 see www.fischer-international.com
European Assessment Document for plastic anchors
made of virgin or non-virgin material for fixing of
external thermal insulation composite systems with
rendering, 2017
7 Environmental Product Declaration fischerwerke GmbH & Co. KG – Insulation fixings
Publisher
Institut Bauen und Umwelt e.V. Tel +49 (0)30 3087748- 0
Panoramastr. 1 Fax +49 (0)30 3087748- 29
10178 Berlin Mail info@ibu-epd.com
Germany Web www.ibu-epd.com
Programme holder
Institut Bauen und Umwelt e.V. Tel +49 (0)30 - 3087748- 0
Panoramastr 1 Fax +49 (0)30 – 3087748 - 29
10178 Berlin Mail info@ibu-epd.com
Germany Web www.ibu-epd.com
Author of the Life Cycle
Assessment Tel +49 (0)711 341817-0
Sphera Solutions GmbH Fax +49 (0)711 341817-25
Hauptstraße 111- 113 Mail info@sphera.com
70771 Leinfelden-Echterdingen Web www.sphera.com
Germany
Owner of the Declaration
fischerwerke GmbH & Co. KG Tel +49 (0)7443 12-0
Klaus-Fischer-Straße 1 Fax +49 (0)7443 12-4222
72178 Waldachtal Mail info@fischer.de
Germany Web www.fischer.de
