ENVIRONMENTAL PRODUCT DECLARATION
as per ISO 14025 and EN 15804+A2
Owner of the Declaration dormakaba International Holding GmbH
Publisher Institut Bauen und Umwelt e.V. (IBU)
Programme holder Institut Bauen und Umwelt e.V. (IBU)
Declaration number EPD-DOR-20240126-CBA1-EN
Issue date 15/07/2024
Valid to 14/07/2029
Mortise Lock Saflok Quantum Pixel
dormakaba
www.ibu-epd.com | https://epd-online.com
General Information
dormakaba Mortise Lock Saflok Quantum Pixel
Programme holder Owner of the declaration
IBU – Institut Bauen und Umwelt e.V. dormakaba International Holding GmbH
Hegelplatz 1 DORMA Platz 1
10117 Berlin 58256 Ennepetal
Germany Germany
Declaration number Declared product / declared unit
EPD-DOR-20240126-CBA1-EN 1 piece of the product: Saflok Quantum Pixel consisting of the following
items:
• Mortise Lock Saflok Quantum Pixel
• Lever handle
• Fixing materials
• Product packaging
This declaration is based on the product category rules: Scope:
Electronic and physical Access Control Systems, 01/08/2021 This Environmental Product Declaration refers to a specific mortise lock
(PCR checked and approved by the SVR) manufactured by dormakaba. The EPD is representative for the Saflok
Quantum Pixel Series. The production site is located in Montreal (Canada).
Issue date Data represents the year 2023.
The owner of the declaration shall be liable for the underlying information
15/07/2024
and evidence; the IBU shall not be liable with respect to manufacturer
information, life cycle assessment data and evidences.
Valid to
The EPD was created according to the specifications of EN 15804+A2. In
14/07/2029 the following, the standard will be simplified as EN 15804.
Verification
The standard EN 15804 serves as the core PCR
Independent verification of the declaration and data according to ISO
14025:2011
internally X externally
Dipl.-Ing. Hans Peters
(Chairman of Institut Bauen und Umwelt e.V.)
Florian Pronold Matthias Klingler,
(Managing Director Institut Bauen und Umwelt e.V.) (Independent verifier)
1 Environmental Product Declaration - dormakaba - Mortise Lock Saflok Quantum Pixel
Product
Performance data of the product with respect to its
Product description/Product definition characteristics in accordance with the relevant technical
Saflok Quantum Pixel is the newest addition to dormakaba's provision which can be applied are mentioned above.
award-winning Quantum Series of RFID electronic locks. The
Quantum Pixel provides an easy-to use, secure, and flexible
solution that is both visually attractive and high-performing. Base materials/Ancillary materials
With its electronics concealed within the door, the Quantum The major material composition including the packaging of the
Pixel's visible hardware is minimal resulting in a lock design product is listed below:
that integrates seamlessly with any hotel decor. Name Value Unit
Steel 45 %
For the use and application of the product the representative
Zinc 19 %
national provisions apply. For the Saflok Quantum Pixel the
standards which can be applied are the following: Paper 15 %
Stainless steel 9 %
• ANSI A156.13
• ANSI A156.25 Electronics 5 %
• UL 10C Brass 3 %
• ULC CAN S-104 Plastics 2 %
• EN 14846
The product includes partial articles which contain substances
• EN 1634-1
listed in the Candidate List of REACH Regulation
• EN 1363-1
1907/2006/EC (date: 23.01.2024) exceeding 0.1 percentage by
mass: yes
Application
The mortise lock Saflok Quantum Pixel is ideal for new • Lead (Pb): 7439-92-1 (CAS-No.) is included in some of
construction projects or in case that doors need to be replaced. the alloys used. The concentration of lead in each
The lock series is suitable for small to very large-scale hotels. individual alloy does not exceed 4 % (by mass).
The mortise locks are for interior doors only. One application is
the access control for quest rooms. The Candidate List can be found on the ECHA website
address: https:echa.europa.eu/de/home.
Technical Data
The Saflok Quantum Pixel has following technical properties: Reference service life
The reference service life for the Saflok Quantum Pixel Series
Name Value Unit amounts to 10 years, depending on the application and
Reader cover polycarbonate color: black, white frequency of use. For repairs and renewals, suitable spare
parts are available. The mortise lock series is tested and
ADA standard bright chrome, bright brass,
finish certified to BHMA A156.13, meaning they are designed to
levers satin chrome, satin brass
withstand a minimum of 1.000.000 cycles.
Door thickness minimum 1,38" (35,1 mm)
Door thickness maximum 3,0" (77 mm)
ANSI lock case locking option with 1" lock front mortise
RFID
options Mifare Classic and Mifare Plus
credentials
LCA: Calculation rules
Production - Module A1-A3
Declared Unit The product stage includes: — A1, raw material extraction,
processing and mechanical treatments, processing of
The declared unit is 1 piece of the product: Quantum pixel secondary material input (e.g. recycling processes), — A2,
including packaging transport to the manufacturer, — A3, manufacturing and
Name Value Unit assembly including provision of all materials, products and
energy, as well as waste processing up to the end-of-waste
Declared unit 1 piece/product
state.
Mass of declared product 3.5 kg
Mass of packaging 0,542 kg
Construction stage - Modules A4-A5
Other declared units are allowed if the conversion is shown The construction process stage includes:
transparently. — A4, transport to the building site; — A5, installation into the
building; including provision of all materials, products and
energy, as well as waste processing up to the end-of-waste
state or disposal of final residues during the construction
System boundary process stage.
The type of EPD is: cradle to gate with options, modules C1– Maintenance – Module B2
C4, and module D (A1–A3 + C + D and additional modules: This module includes the production and the end of life of the
A4+ A5) batteries. The potential use of batteries is declared in module
B2.
2 Environmental Product Declaration - dormakaba - Mortise Lock Saflok Quantum Pixel
Land or region, in which the declared product system is
End-of-life stage– Modules C1-C4 and D manufactured, used or handled at the end of the product´s
The end-of-life stage includes: — C1, de-construction, lifespan: Global
demolition: — C2, transport to waste processing; — C3, waste
processing for reuse, recovery and/or recycling; — C4,
disposal; including provision and all transport, provision of all Comparability
materials, products and related energy and water use. Module Basically, a comparison or an evaluation of EPD data is only
D (Benefits and loads beyond the system boundary) includes: possible if all the data sets to be compared were created
— D, recycling potentials, expressed as net impacts and according to EN 15804 and the building context, respectively
benefits. the product-specific characteristics of performance, are taken
into account. Background database: GaBi, SP40.
Geographic Representativeness
LCA: Scenarios and additional technical information
batteries are provided by dormakaba. During the operation of
Characteristic product properties of biogenic carbon the product, the only energy consumption comes from the
battery use. The battery must be exchanged on average 5
Information on describing the biogenic carbon content at times over the declared service life.
factory gate
In order to allow scaling, the exchange of 1 battery is declared
Name ValueUnit
in the LCA.
kg
Biogenic carbon content in product -
C
Biogenic carbon content in accompanying kg
0.19 Reference service life
packaging C
Name Value Unit
Note: 1 kg of biogenic carbon is equivalent to 44/12 kg of CO2
Life Span according to the manufacturer 10 a
End of life (C1-C4)
C1: The product dismantling from the building is done manually
without environmental burden.
Transport to the building site (A4) C2: Transport to waste management is 50 km.
Name Value Unit Name Value Unit
Liters of fuel 0,00276 l/100km Collected separately waste type waste type 2.96 kg
Transport distance 100 km Recycling 2.78 kg
Capacity utilisation (including empty runs) 55 % Energy recovery 0.04 kg
The product is transported via truck. The product is stored in Landfilling 0.142 kg
the dormakaba logistic center in Montreal. The main distribution The product is disassembled in a recycling process. Material
region is North America. In order to allow scaling to a specific recycling is then assumed for metals and electronics. The
point of installation 100 km are declared. plastic components are assumed to be incinerated with energy
recovery. The batteries and minor proportions of residues
Installation into the building (A5) arising from the recycling process are landfilled. Region for the
End of Life is: Global.
Name Value Unit
Waste packaging (paper and plastic) 0,542 kg
Reuse, recovery and/or recycling potentials (D), relevant
Maintenance (B2) scenario information
Name Value Unit Name Value Unit
Maintenance cycle 5 Number/RSL Recycling 100 %
dormakaba Mortise Lock Quantum Pixel series are operated The collection rate is 100 %.
using a battery and are not connected to mains electricity. The
3 Environmental Product Declaration - dormakaba - Mortise Lock Saflok Quantum Pixel
LCA: Results
DESCRIPTION OF THE SYSTEM BOUNDARY (X = INCLUDED IN LCA; MND = MODULE OR INDICATOR NOT DECLARED; MNR
= MODULE NOT RELEVANT)
Benefits and
Construction loads beyond
Product stage Use stage End of life stage
process stage the system
boundaries
la ire ta m w a Ry lp p u s tro p s n a rT g n iru tc a fu n a M e h t m o rf tro p s n a rTe tis e h t o t e ta g y lb m e s s A e s U e c n a n e tn ia M ria p e R tn e m e c a lp e R tn e m h s ib ru fe R y g re n e la n o ita re p Oe s u re ta w la n o ita re p Oe s u n o itc u rts n o c -e Dn o itilo m e d tro p s n a rT g n is s e c o rp e ts a W la s o p s iD -e s u e R-y re v o c e R-g n ilc y c e Rla itn e to p
A1 A2 A3 A4 A5 B1 B2 B3 B4 B5 B6 B7 C1 C2 C3 C4 D
X X X X X MND X MNR MNR MNR MND MND X X X X X
RESULTS OF THE LCA - ENVIRONMENTAL IMPACT according to EN 15804+A2: 1 piece Saflok Quantum Pixel
Parameter Unit A1-A3 A4 A5 B2 C1 C2 C3 C4 D
GWP-total kg CO 2 eq 5.4E+01 3.1E-02 7.84E-01 2.09E-01 0 1.6E-02 1.81E-01 2E-03 -4.66E+00
GWP-fossil kg CO 2 eq 5.45E+01 2.9E-02 5.3E-02 2.09E-01 0 1.6E-02 1.81E-01 2E-03 -4.66E+00
GWP-biogenic kg CO 2 eq -6.24E-01 1E-03 7.31E-01 2.88E-04 0 7.26E-04 4.22E-06 7.34E-06 2E-03
GWP-luluc kg CO 2 eq 5.7E-02 6.96E-07 1.43E-05 8.67E-05 0 3.74E-07 1.02E-05 6.18E-06 -6E-03
ODP kg CFC11 eq 3.11E-09 3.09E-18 1.53E-16 7.19E-16 0 1.66E-18 9.14E-17 7.96E-18 -1.97E-14
AP mol H+ eq 3.77E-01 2.93E-05 2.16E-04 2.11E-03 0 1.57E-05 3.23E-05 1.54E-05 -3.4E-02
EP-freshwater kg P eq 2.9E-04 6.26E-09 2.92E-08 1.48E-07 0 3.36E-09 1.46E-08 3.69E-09 -8.61E-06
EP-marine kg N eq 6.59E-02 9.32E-06 7.72E-05 2.54E-04 0 5.01E-06 7.27E-06 3.96E-06 -4E-03
EP-terrestrial mol N eq 7.05E-01 1.04E-04 9.73E-04 2.32E-03 0 5.56E-05 1.47E-04 4.36E-05 -4.1E-02
kg NMVOC
POCP 1.91E-01 2.64E-05 2.05E-04 7.85E-04 0 1.42E-05 2.01E-05 1.2E-05 -1.3E-02
eq
ADPE kg Sb eq 2.01E-02 8.78E-10 2.37E-09 9.05E-06 0 4.71E-10 1.25E-09 1.93E-10 -2E-03
ADPF MJ 6.45E+02 4.15E-01 2.53E-01 2.37E+00 0 2.23E-01 8.4E-02 2.8E-02 -6.33E+01
m3 world eq
WDP 1.24E+01 5.73E-05 9.7E-02 2.3E-02 0 3.08E-05 1.9E-02 2.25E-04 -1.44E+00
deprived
GWP = Global warming potential; ODP = Depletion potential of the stratospheric ozone layer; AP = Acidification potential of land and water; EP =
Eutrophication potential; POCP = Formation potential of tropospheric ozone photochemical oxidants; ADPE = Abiotic depletion potential for non-fossil
resources; ADPF = Abiotic depletion potential for fossil resources; WDP = Water (user) deprivation potential)
RESULTS OF THE LCA - INDICATORS TO DESCRIBE RESOURCE USE according to EN 15804+A2: 1 piece Saflok Quantum
Pixel
Parameter Unit A1-A3 A4 A5 B2 C1 C2 C3 C4 D
PERE MJ 1.17E+02 1E-03 6.39E+00 1.97E-01 0 7.03E-04 2.2E-02 4E-03 -1.19E+01
PERM MJ 6.35E+00 0 -6.35E+00 0 0 0 0 0 0
PERT MJ 1.24E+02 1E-03 4.7E-02 1.97E-01 0 7.03E-04 2.2E-02 4E-03 -1.19E+01
PENRE MJ 6.38E+02 4.15E-01 8.38E-01 2.37E+00 0 2.23E-01 6.82E+00 2.8E-02 -6.33E+01
PENRM MJ 7.32E+00 0 -5.85E-01 0 0 0 -6.73E+00 0 0
PENRT MJ 6.45E+02 4.15E-01 2.53E-01 2.37E+00 0 2.23E-01 8.4E-02 2.8E-02 -6.33E+01
SM kg 1.95E+00 0 0 0 0 0 0 0 0
RSF MJ 0 0 0 0 0 0 0 0 0
NRSF MJ 0 0 0 0 0 0 0 0 0
FW m3 3.35E-01 2.35E-06 2E-03 7.23E-04 0 1.26E-06 4.43E-04 7.1E-06 -4.5E-02
PERE = Use of renewable primary energy excluding renewable primary energy resources used as raw materials; PERM = Use of renewable primary
energy resources used as raw materials; PERT = Total use of renewable primary energy resources; PENRE = Use of non-renewable primary energy
excluding non-renewable primary energy resources used as raw materials; PENRM = Use of non-renewable primary energy resources used as raw
materials; PENRT = Total use of non-renewable primary energy resources; SM = Use of secondary material; RSF = Use of renewable secondary fuels;
NRSF = Use of non-renewable secondary fuels; FW = Use of net fresh water
RESULTS OF THE LCA – WASTE CATEGORIES AND OUTPUT FLOWS according to EN 15804+A2:
1 piece Saflok Quantum Pixel
Parameter Unit A1-A3 A4 A5 B2 C1 C2 C3 C4 D
HWD kg 2.55E-05 4.03E-11 4.1E-10 1.15E-08 0 2.16E-11 3.2E-10 4.29E-10 -9.69E-07
NHWD kg 1.86E+00 4.25E-05 2.7E-02 1E+00 0 2.28E-05 1.9E-02 1.42E-01 -1.8E-01
RWD kg 1.7E-02 4.46E-07 1.3E-05 4.87E-05 0 2.39E-07 3.12E-06 3.21E-07 -2E-03
CRU kg 0 0 0 0 0 0 0 0 0
MFR kg 0 0 0 0 0 0 2.78E+00 0 0
MER kg 0 0 0 0 0 0 0 0 0
EEE MJ 0 0 1.2E+00 0 0 0 1.18E+00 0 0
EET MJ 0 0 2.2E+00 0 0 0 2.75E+00 0 0
4 Environmental Product Declaration - dormakaba - Mortise Lock Saflok Quantum Pixel
HWD = Hazardous waste disposed; NHWD = Non-hazardous waste disposed; RWD = Radioactive waste disposed; CRU = Components for re-use;
MFR = Materials for recycling; MER = Materials for energy recovery; EEE = Exported electrical energy; EET = Exported thermal energy
RESULTS OF THE LCA – additional impact categories according to EN 15804+A2-optional:
1 piece Saflok Quantum Pixel
Parameter Unit A1-A3 A4 A5 B2 C1 C2 C3 C4 D
Disease
PM 3.72E-06 1.54E-10 1.24E-09 1.52E-08 0 8.27E-11 4.12E-10 1.91E-10 -4.07E-07
incidence
IR kBq U235 eq 1.8E+00 6.37E-05 2E-03 5.24E-03 0 3.42E-05 2.81E-04 3.3E-05 -2.36E-01
ETP-fw CTUe 2.7E+02 2.94E-01 1.18E-01 6.06E-01 0 1.58E-01 3.2E-02 1.6E-02 -2.98E+01
HTP-c CTUh 4.91E-07 5.53E-12 6.46E-12 5.97E-11 0 2.97E-12 2.73E-12 2.38E-12 5.3E-09
HTP-nc CTUh 1.08E-06 2.37E-10 3.1E-10 3.41E-09 0 1.27E-10 2.76E-10 2.63E-10 9.79E-07
SQP SQP 1.89E+02 1E-03 6.8E-02 4.61E-01 0 5.73E-04 2.5E-02 6E-03 -1.13E+01
PM = Potential incidence of disease due to PM emissions; IR = Potential Human exposure efficiency relative to U235; ETP-fw = Potential comparative
Toxic Unit for ecosystems; HTP-c = Potential comparative Toxic Unit for humans (cancerogenic); HTP-nc = Potential comparative Toxic Unit for humans
(not cancerogenic); SQP = Potential soil quality index
Disclaimer 1 – for the indicator “Potential Human exposure efficiency relative to U235”. This impact category deals mainly with the
eventual impact of low-dose ionizing radiation on human health of the nuclear fuel cycle. It does not consider effects due to possible
nuclear accidents, occupational exposure or radioactive waste disposal in underground facilities. Potential ionizing radiation from the
soil, radon and from some construction materials is also not measured by this indicator.
Disclaimer 2 – for the indicators “abiotic depletion potential for non-fossil resources”, “abiotic depletion potential for fossil resources”,
“water (user) deprivation potential, deprivation-weighted water consumption”, “potential comparative toxic unit for ecosystems”,
“potential comparative toxic unit for humans – cancerogenic”, “Potential comparative toxic unit for humans - not cancerogenic”,
“potential soil quality index”. The results of this environmental impact indicator shall be used with care as the uncertainties on these
results are high as there is limited experience with the indicator.
This EPD was created using a software tool.
References
ANSI A156.25 REACH
ANSI A156.25:2023, Electrified Locking Devices Regulation (EC) No 1907/2006 of the European Parliament and
of the Council on the Registration, Evaluation, Authorisation
ANSI A156.13 and Restriction of Chemicals (REACH)
ANSI A156.13:2022, Mortise Locks
RoHS
UL 10C Directive on the restriction of the use of certain hazardous
UL 10C:2016-06, Standard for Safety Positive Pressure Fire substances in electrical and electronic equipment (RoHS)
Tests of Door Assemblies Directive (EU) No 2011/65
ULC CAN-S104 Further References
ULC CAN-S104:2020-08, Standard Method for Fire Tests of
Door Assemblies IBU 2021
General Instructions for the EPD programme of Institut Bauen
EN 14846 und Umwelt e.V. Version 2.0, Berlin: Institut Bauen und Umwelt
EN 14846:2008-11 Building hardware - Locks and e.V., 2021. www.ibu-epd.com
latches - Electromechanically operated locks and striking
plates - Requirements and test methods GaBi
Sphera Solutions GmbH
EN 1634-1 Gabi Software System and Database for Life Cycle Engineering
EN 1634-1:2018-04, Fire resistance and smoke control tests for 19922020
door and shutter assemblies, openable windows and elements Version 10.0.0.71
of building hardware University of Stuttgart
Leinfelden-Echterdingen
EN 1363-1
EN 1363-1:2020-05, Fire resistance tests - Part 1: General GaBi ts documentation
Requirements GaBi life cycle inventory data documentation
(https://www.gabisoftware.com/support/gabi/gabidatabase-
ISO 14025 2020-lcidocumentation/).
ISO 14025:2011-10, Environmental labels and declarations —
Type III environmental declarations — Principles and LCA-tool dormakaba
procedures LCA too, ESC
Tool No.: IBU-DOR-202109-LT1-EN.
EN 15804 Developed by Sphera Solutions GmbH
EN 15804:2019+A2,
Sustainability of construction works — Environmental Product PCR Part A
Declarations — Core rules for the product category of PCR – Part A: Calculation Rules for the Life Cycle Assessment
construction products and Requirements on the Project Re-port according to EN
15804+A2:2019, Version 1.0, 2020, Institut Bauen und Umwelt
5 Environmental Product Declaration - dormakaba - Mortise Lock Saflok Quantum Pixel
e.V., www.ibu-epd.com. Bauen und Umwelt e.V., www.ibu-epd.com.
PCR Part B
PCR – Part B: Requirements on the EPD for Electronic and
physical Access Control Systems, version 08/2021, Institut
6 Environmental Product Declaration - dormakaba - Mortise Lock Saflok Quantum Pixel
Publisher
Institut Bauen und Umwelt e.V. +49 (0)30 3087748- 0
Hegelplatz 1 info@ibu-epd.com
10117 Berlin www.ibu-epd.com
Germany
Programme holder
Institut Bauen und Umwelt e.V. +49 (0)30 3087748- 0
Hegelplatz 1 info@ibu-epd.com
10117 Berlin www.ibu-epd.com
Germany
Author of the Life Cycle Assessment
dormakaba International Holding GmbH +49 2333 793-0
DORMA Platz 1 info.de@dormakaba.com
58256 Ennepetal www.dormakaba.com
Germany
Owner of the Declaration
dormakaba International Holding GmbH +49 2333 793-0
DORMA Platz 1 info.de@dormakaba.com
58256 Ennepetal www.dormakaba.com
Germany
7 Environmental Product Declaration - dormakaba - Mortise Lock Saflok Quantum Pixel
