ENVIRONMENTAL PRODUCT DECLARATION
as per ISO 14025 and EN 15804+A1
Owner of the Declaration Etex Building Performance International
Programme holder Institut Bauen und Umwelt e.V. (IBU)
Publisher Institut Bauen und Umwelt e.V. (IBU)
Declaration number EPD-PMT-20210294-IBC1-EN
Issue date 23.11.2021
Valid to 22.11.2026
PROMATECT®-L500
Medium density calcium silicate fire protective boards
Promat
www.ibu-epd.com | https://epd-online.com
Umwelt Produktdeklaration Name des Herstellers – Name des Produkts
1. General Information
Etex Building Performance NV PROMATECT®-L500
Programme holder Owner of the declaration
IBU – Institut Bauen und Umwelt e.V. Etex Building Performance International
Panoramastr. 1 500 Rue Marcel Demonque
10178 Berlin F-84915 Avignon
Germany France
Declaration number Declared product / declared unit
EPD-PMT-20210294-IBC1-EN The functional unit is 1 m² of PROMATECT®-L500 with
a thickness of 30 mm.
This declaration is based on the product Scope:
category rules: The life cycle assessment is based on production data
Calcium silicate insulating materials, 11.2017 of PROMATECT®-L500 of the year 2019 at the
(PCR checked and approved by the SVR) production site Tisselt, Belgium.
Issue date The owner of the declaration shall be liable for the
23.11.2021 underlying information and evidence; the IBU shall not
be liable with respect to manufacturer information, life
cycle assessment data and evidences.
Valid to
The EPD was created according to the specifications
22.11.2026
of EN 15804+A1. In the following, the standard will be
simplified as EN 15804.
Verification
The standard EN 15804 serves as the core PCR
Independent verification of the declaration and data
according to ISO 14025:2010
Dipl. Ing. Hans Peters internally x externally
(chairman of Institut Bauen und Umwelt e.V.)
Dr. Alexander Röder Vito D'Incognito
(Managing Director Institut Bauen und Umwelt e.V.)) (Independent verifier)
2. Product
2.1 Product description/Product definition 2.3 Technical Data
PROMATECT®-L500 is a lightweight, non-
combustible, fire-resisting calcium silicate board, not
sensitive to moisture.
Constructional data
For the placing of the product on the market in the
European Union/European Free Trade Association
EU/EFTA (with the exception of Switzerland) the Name Value Unit
Regulation (EU) No. 305/2011 (CPR) applies. The Gross density 23°C, 50%RH;
500 kg/m3
product needs a declaration of performance taking into according to ETA 06/0218
consideration ETA 06/0218_2018-06- Compressive strength according
4.2 N/mm2
25_PROMATECT®-L500 and the CE-marking. For the to EN 826
application and use the respective national provisions Tensile strength (perpendicular)
0.057 N/mm2
apply. according to EN 1607
Flexural strength according to EN
1.7 N/mm2
2.2 Application 12467
PROMATECT®-L500 is primarily used in interior Thermal conductivity according to
0.09 W/(mK)
building applications where normal to high levels of fire EN 12667
resistance are required. Water vapour diffusion resistance
The board is intended to protect elements or to be factor according to EN 12572 3.2 -
used in technical services assemblies. Main uses are Tensile strength (parallel)
the construction of fire resistant ducts, cladding of according to EN 1608 445 kPa
sheet metal ducts and providing fire rated cable and
Values are guidance values and do not reflect a
service enclosures.
statistical evaluation or guaranteed value.
2 Environmental Product Declaration Etex Building Performance NV – PROMATECT®-L500
Performance data of the product in accordance with manufacturing plant adheres to the Belgium
the declaration of performance with respect to its environmental and health and safety regulations.
essential characteristics according to ETA 06/0218.
2.8 Product processing/Installation
2.4 Delivery status The fire protective board is cut and machined using
PROMATECT®-L500 fire protective calcium silicate conventional woodworking equipment.
boards are available in 1200 x 2500 mm in Fixing the boards will require appropriate means,
20,25,30,35,40,50,52 and 60 mm and available in which will depend upon the application and bearing
1220 x 2440 in 50 mm. structure. Boards can be installed using screws or
glues.
2.5 Base materials/Ancillary materials Industrial and environmental protection are assured
Main raw materials used (in weight percentages): through training and coaching staff on safety and
- sand: 25-45 % environmental impacts. Dust levels are kept low by
- lime: 25-45 % performing dust extraction. Noise is reduced by noise
- cement: <25 % insulation on the machines and ear protection is
- fibres: <6 % provided for persons entering the production area.
Reaction is performed in an aqueous suspension. Regular measurements on noise and dust are
performed and show conformity to the permitted
This article contains substances listed in the candidate levels.
list (date: 19.01.2021) exceeding 0.1 percentage by All national, local and other applicable safety
mass: no. regulations are complied with.
This article contains other carcinogenic, mutagenic,
reprotoxic (CMR) substances in categories 1A or 1B 2.9 Packaging
which are not on the candidate list, exceeding 0.1 All fire protection boards are packed onto wooden
percentage by mass: no. pallets, wrapped with polyester strapping tape and
Biocide products were added to this construction strengthened with cardboard corners.
product or it has been treated with biocide products
(this then concerns a treated product as defined by the
(EU) Ordinance on Biocide Products No. 528/2012): 2.10 Condition of use
no. PROMATECT®-L500 boards are resistant to the
effects of moisture and will not physically deteriorate
when used in damp or humid conditions. Performance
2.6 Manufacture characteristics are not degraded by age or moisture.
Sand, water and lime are mixed and blended in a Boards do not encourage mould growth and are
reactor to form calcium silicate. This is combined in a resistant to attacks by insects or vermin.
mixer with the other raw materials to form a thick
slurry. The slurry is formed to a board in a filter press. 2.11 Environment and health during use
Boards are dried, edges are trimmed and the upper PROMATECT®-L500 boards are chemically inert.
surface is sanded to the specific thickness. All material When the products are used as designed, the current
which is cut off or sanded away is fully recycled within state of knowledge indicates that there is no risk
the process. involved for the environment or health.
2.12 Reference service life
The service life according to the "Bundesinstitut für
Bau-, Stadt- und Raumforschung" (BBSR) table is
indicated to be ≥ 50 years.
The reference service life (RSL) is therefore estimated
to be 50 years. This RSL corresponds to the period
after which a building renovation is usually needed,
independently of the actual lifetime of the product
(which can be longer than 50 years).
2.13 Extraordinary effects
Fire
The PROMATECT®-L500 boards have a reaction to
The quality management system of the company and
fire classification A1 or non-combustible according to
the production facility are certified according to ISO
EN13501-1.
9001.
Fire protection
2.7 Environment and health during
Name Value
manufacturing
Building material class A1
Promat commits to a clean, healthy and safe working
Burning droplets -
environment for every person working in and for the
Smoke gas development -
company.
The company and the manufacturing site have an
Water
environment, health and safety management system
All ingredients are firmly bound in the matrix. The
which is ISO 14001 and ISO 45001 certified. The
boards are insensitive to moisture and no ingredients
3 Environmental Product Declaration Etex Building Performance NV – PROMATECT®-L500
which could be hazardous to water are washed out in For this EPD, a conservative worst-case scenario was
the event of extraordinary effects by water. chosen at the end-of-life stage and the product was
sent for 100% to landfill.
Mechanical destruction
In order to prevent any reduction of fire performance 2.15 Disposal
following unforeseeable mechanical destruction, all Within the production process, generated waste is re-
damage of the components needs to be repaired using used within the process.
materials specified by ETA 06/0218. When after end-of-life reusing or recycling the boards
Besides the need for repair, the destruction will not as described in the previous paragraph is not practical,
have any significant environmental impact. the boards can be disposed to landfill without pre-
treatment thanks to the largely mineral ingredients
2.14 Re-use phase resulting in an inert matrix, The waste code in
Several possibilities exist for the boards after the end- accordance with the European List of Waste is
of-life of the application in which they were used. 170904.
If the boards are removed non-destructively by
releasing the screws, the undamaged product can be 2.16 Further information
re-used in accordance with the original purpose. Further information is available on the following web
If not contaminated with other building construction site :
material, the boards also allow being recycled by the https://www.promat.com
manufacturer.
Furthermore, the products referred to could be used as
filler and bulk material in civil engineering, as an
absorber in cat litter or be recycled in the cement
industry.
3. LCA: Calculation rules
3.1 Declared Unit Adjustment factor to 1 m² 60 mm
(multiply results by this factor to 2.00 -
The declared unit is 1 m² of PROMATECT®-L500 with obtain the results for 1 m² 60 mm)
a thickness of 30 mm.
In an annexe to this EPD, the LCA results for the
thickness 50 mm are declared as well.
The results for other thicknesses can be obtained by
multiplying the presented results by the corresponding 3.2 System boundary
adjustment factor as included in the table. Type of the EPD: cradle to grave.
The following life cycle stages and modules are
Declared unit included:
Name Value Unit
Gross density 490 kg/m3 Production stage (A1-A3):
Declared unit 1.00 m²  pre-chains of the raw materials and their
Grammage 14.7 kg/m² transportation to the manufacturing site
Conversion factor to 1 kg (divide
 energy consumption during production
results by this factor to obtain the 14.7 -
 recycling and disposal of production wastes
results for 1 kg)
Adjustment factor to 1 ton  production of packaging
(multiply results by this factor to 68.03 -
obtain the results for 1 ton)
Adjustment factor to 1 m² 15 mm Construction stage (A4-A5):
(multiply results by this factor to 0.50 -  transportation of product to the construction
obtain the results for 1 m² 15 mm)
site
Adjustment factor to 1 m² 20 mm
 disposal of installation wastes
(multiply results by this factor to 0.67 -
obtain the results for 1 m² 20 mm)  incineration of packaging materials (potential
Adjustment factor to 1 m² 25 mm benefits from energy substitution within the
(multiply results by this factor to 0.83 - incineration process are declared in module
obtain the results for 1 m² 25 mm) D)
Adjustment factor to 1 m² 35 mm
(multiply results by this factor to 1.17 -
obtain the results for 1 m² 35 mm)
Use stage (B1-B7):
Adjustment factor to 1 m² 40 mm
 efforts for the use of the product,
(multiply results by this factor to 1.33 -
obtain the results for 1 m² 40 mm) maintenance and operational efforts
Adjustment factor to 1 m² 50 mm  modules B3, B4, B5 are declared as MNR
(multiply results by this factor to 1.67 - (module not relevant) according to the IBU
obtain the results for 1 m² 50 mm) requirement. These modules are defined on
Adjustment factor to 1 m² 52 mm
building level in general
(multiply results by this factor to 1.73 -
obtain the results for 1 m² 52 mm)
4 Environmental Product Declaration Etex Building Performance NV – PROMATECT®-L500
End-of-life stage (C1-C4): 3.5 Background data
 transport to disposal of the material Background data were sourced from GaBi 10 database
 landfill end-of-life scenario was considered version 2021.
3.6 Data quality
This study is mainly based on primary data collected
Loads and benefits beyond system boundary (D): directly from the manufacturing site and therefore data
 loads and benefits from the recycling of quality can be assumed to be very good.
production waste and incineration of The last update of the GaBi database used for
packaging waste the background data was February 2021.
3.7 Period under review
Data for the entire production period of 2019 were
3.3 Estimates and assumptions
collected and used for this EPD.
Most of the input and output influences of the Life
Cycle Inventory Analysis could be depicted using
3.8 Allocation
corresponding data from the GaBi database.
Allocation in background data
Assumptions and approximations were applied in case
Specific information on allocation within the
of a lack of representative data.
background data is given in the GaBi documentation.
There were no data records in the GaBi database
Allocation in foreground data
available for the wooden pallets, they were
The production process does not deliver any co-
approximated using the "Solid construction timber"
products. In modules A1 to A3, specific raw material
dataset.
and transport data were available, energy, waste and
The waste water treatment of process water was
water could not be directly allocated to the product and
approximated by datasets of municipal waste water
were allocated via the production volume of the
treatment, which will result in an overestimation of
specific products.
impacts.
Allocation for waste materials
All assumptions and approximations were documented
The environmental burden of the incineration of
precisely.
packaging in the construction process stage is
assigned to the system (A5); resulting credits for
thermal and electrical energy are declared in module
3.4 Cut-off criteria
D.
In the assessment, all utilised raw material, thermal
energy and electric power were considered using
GaBi datasets. Only the transport of packaging,
3.9 Comparability
production waste to recycling/disposal and of
Basically, a comparison or an evaluation of EPD data
installation loss waste to recycling was cut-off in this
is only possible if all the data sets to be compared
study.
were created according to EN 15804 and the building
Production of capital equipment, facilities and
context, respectively the product-specific
infrastructure required for the manufacture are outside
characteristics of performance, are taken into account.
the scope of the study and thus were not included.
GaBi database version 2021.1 serves as a
background database for the calculation of the life
cycle assessment.
4. LCA: Scenarios and additional technical information
VOC in the air 0 kg
Transport to the building site (A4)
For the transport from the factory gate to the building Use or application of the installed product (B1) see
site, an average distance of 100km was assumed. This section 2.12 "Use"
distance can be assumed to be representative of No efforts and releases of substances occur during
deliveries within Belgium. the normal (i.e. anticipated) use phase.
Name Value Unit
Name Value Unit
Litres of fuel 0.031 l/100km Maintenance (B2)
Transport distance 100 km No efforts occur during maintenance.
Capacity utilisation (including empty Name Value Unit
61 %
runs) Number/
Maintenance cycle 0
Gross density of products transported 490 kg/m3 RSL
Water consumption 0 m3
Auxiliary 0 kg
Other resources 0 kg
Installation into the building (A5) Electricity consumption 0 kWh
Only waste treatment of installation loss and packaging Other energy carriers 0 MJ
is considered in this module. Material loss 0 kg
Installation into the building (A5)
Name Value Unit Repair (B3)
Material loss 0.74 kg Name Value Unit
5 Environmental Product Declaration Etex Building Performance NV – PROMATECT®-L500
Information on the repair process - - Although re-use and recycling of the PROMATECT®-
Information on the inspection process - - L500 is possible, this is not yet a widely established
Number/ practice. Therefore, no possible benefits of recycling or
Repair cycle -
RSL re-use of the boards were taken into account in this
Water consumption - m3 study. In module D, only the benefits from recycling of
Auxiliary - kg production waste and incineration of waste packaging
Other resources - kg were taken into account.
Name Value Unit
Electricity consumption - kWh
Exported electrical energy 1.8 MJ
Other energy carriers - MJ
Exported thermal energy 3.2 MJ
Material loss - kg
Replacement (B4) / Refurbishment (B5)
Name Value Unit
Number/
Replacement cycle -
RSL
Electricity consumption - kWh
Litres of fuel - l/100km
Replacement of worn parts - kg
Reference service life
Name Value Unit
Reference service life - a
Life Span (according to BBSR) >=50 a
Life Span according to the
- a
manufacturer
Declared product properties (at the
- -
gate) and finishes
Design application parameters (if
instructed by the manufacturer),
including the references to the - -
appropriate practices and application
codes
An assumed quality of work, when
installed in accordance with the - -
manufacturer’s instructions
Outdoor environment, (for outdoor
applications), e.g. weathering,
pollutants, UV and wind exposure, - -
building orientation, shading,
temperature
Indoor environment (for indoor
applications), e.g. temperature, - -
moisture, chemical exposure
Usage conditions, e.g. frequency of
- -
use, mechanical exposure
Maintenance e.g. required frequency,
type and quality and replacement of - -
components
Operational energy use (B6) and Operational water
use (B7)
No efforts occur in modules B6 and B7.
Name Value Unit
Water consumption 0 m3
Electricity consumption 0 kWh
Other energy carriers 0 MJ
Equipment output 0 kW
End-of-life (C1-C4)
A conservative approach was used in this study.
Although after end-of-life, scenarios where the
boards are re-used or recycled are realistic, a
scenario with 100% landfill was used.
Name Value Unit
Landfilling 14.7 kg
Re-use, recovery and/or recycling potentials (D),
relevant scenario information
6 Environmental Product Declaration Etex Building Performance NV – PROMATECT®-L500
5. LCA: Results
The following tables depict the results of the indicators for the Life Cycle Assessment, use of resources and waste
with reference to 1 m² of PROMATECT®-L500.
DESCRIPTION OF THE SYSTEM BOUNDARY (X = INCLUDED IN LCA; MND = MODULE NOT DECLARED;
MNR = MODULE NOT RELEVANT)
BENEFITS AND
CONSTRUCTI LOADS
PRODUCT STAGE ON PROCESS USE STAGE END OF LIFE STAGE BEYOND THE
STAGE SYSTEM
BOUNDARIES
7 Environmental Product Declaration Etex Building Performance NV – PROMATECT®-L500
lairetam
waR
ylppus tropsnarT
gnirutcafunaM
eht
morf
tropsnarT
etis
eht
ot
etag
ylbmessA esU
ecnanetniaM
riapeR
tnemecalpeR tnemhsibrufeR
ygrene
lanoitarepO esu
retaw
lanoitarepO esu
noitcurtsnoc-eD
noitilomed tropsnarT
gnissecorp
etsaW
lasopsiD -esueR -yrevoceR -gnilcyceR laitnetop
A1 A2 A3 A4 A5 B1 B2 B3 B4 B5 B6 B7 C1 C2 C3 C4 D
X X X X X X X MNR MNR MNR X X X X X X X
RESULTS OF THE LCA - ENVIRONMENTAL IMPACT according to EN 15804+A1: 1 m² 30mm
PROMATECT®-L500
Parameter Unit A1 A2 A3 A4 A5 B1 B2 B6 B7 C1 C2 C3 C4 D
GWP [kg CO2-Eq.] 9.41E+02.54E-11.08E+19.99E-22.28E+00.00E+00.00E+00.00E+00.00E+00.00E+04.78E-20.00E+02.11E-1-4.09E-1
6.09E- 1.39E- 2.67E- 5.83E- 1.28E- 1.15E- -6.35E-
ODP [kg CFC11-Eq.] 1.17E-8 0.00E+00.00E+00.00E+00.00E+00.00E+0 0.00E+0
17 12 17 10 17 15 15
AP [kg SO2-Eq.] 1.55E-2 1.81E-3 6.28E-3 7.93E-5 1.37E-30.00E+00.00E+00.00E+00.00E+00.00E+03.79E-50.00E+01.26E-3-4.29E-4
EP [kg (PO4)3--Eq.] 2.13E-3 2.22E-4 1.70E-3 1.56E-5 2.38E-40.00E+00.00E+00.00E+00.00E+00.00E+07.46E-60.00E+01.43E-4-6.42E-5
POCP [kg ethene-Eq.] 2.15E-3 9.07E-5 9.61E-4-1.00E-61.75E-40.00E+00.00E+00.00E+00.00E+00.00E+0-4.79E-70.00E+09.67E-5-4.41E-5
ADPE [kg Sb-Eq.] 1.02E-6 1.97E-8 1.43E-6 9.01E-9 1.28E-70.00E+00.00E+00.00E+00.00E+00.00E+04.31E-90.00E+02.12E-8-7.26E-8
-
ADPF [MJ] 5.83E+13.34E+01.95E+21.34E+01.33E+10.00E+00.00E+00.00E+00.00E+00.00E+06.40E-10.00E+02.86E+0
5.86E+0
GWP = Global warming potential; ODP = Depletion potential of the stratospheric ozone layer; AP = Acidification potential of land and water; EP =
Caption Eutrophication potential; POCP = Formation potential of tropospheric ozone photochemical oxidants; ADPE = Abiotic depletion potential for non-
fossil resources; ADPF = Abiotic depletion potential for fossil resources
RESULTS OF THE LCA - INDICATORS TO DESCRIBE RESOURCE USE according to EN 15804+A1: 1 m²
30mm PROMATECT®-L500
Parameter Unit A1 A2 A3 A4 A5 B1 B2 B6 B7 C1 C2 C3 C4 D
PERE [MJ] 1.72E+1 1.58E-1 1.54E+1 7.78E-2 1.37E+1 0.00E+0 0.00E+0 0.00E+0 0.00E+0 0.00E+0 3.72E-2 0.00E+0 2.65E+0 -1.64E+0
PERM [MJ] 3.04E+0 0.00E+0 1.11E+1 0.00E+0 -1.13E+1 0.00E+0 0.00E+0 0.00E+0 0.00E+0 0.00E+0 0.00E+0 0.00E+0 -2.25E+0 0.00E+0
PERT [MJ] 2.03E+1 1.58E-1 2.65E+1 7.78E-2 2.43E+0 0.00E+0 0.00E+0 0.00E+0 0.00E+0 0.00E+0 3.72E-2 0.00E+0 3.97E-1 -1.64E+0
PENRE [MJ] 6.53E+1 3.38E+0 1.98E+2 1.36E+0 1.39E+1 0.00E+0 0.00E+0 0.00E+0 0.00E+0 0.00E+0 6.49E-1 0.00E+0 2.95E+0 -7.22E+0
PENRM [MJ] 0.00E+0 0.00E+0 9.07E-2 0.00E+0 -9.07E-2 0.00E+0 0.00E+0 0.00E+0 0.00E+0 0.00E+0 0.00E+0 0.00E+0 0.00E+0 0.00E+0
PENRT [MJ] 6.53E+1 3.38E+0 1.98E+2 1.36E+0 1.38E+1 0.00E+0 0.00E+0 0.00E+0 0.00E+0 0.00E+0 6.49E-1 0.00E+0 2.95E+0 -7.22E+0
SM [kg] 1.95E+0 0.00E+0 0.00E+0 0.00E+0 9.74E-2 0.00E+0 0.00E+0 0.00E+0 0.00E+0 0.00E+0 0.00E+0 0.00E+0 0.00E+0 0.00E+0
RSF [MJ] 0.00E+0 0.00E+0 0.00E+0 0.00E+0 0.00E+0 0.00E+0 0.00E+0 0.00E+0 0.00E+0 0.00E+0 0.00E+0 0.00E+0 0.00E+0 0.00E+0
NRSF [MJ] 0.00E+0 0.00E+0 0.00E+0 0.00E+0 0.00E+0 0.00E+0 0.00E+0 0.00E+0 0.00E+0 0.00E+0 0.00E+0 0.00E+0 0.00E+0 0.00E+0
FW [m³] 1.37E-2 1.82E-4 7.12E-2 8.91E-5 7.35E-3 0.00E+0 0.00E+0 0.00E+0 0.00E+0 0.00E+0 4.26E-5 0.00E+0 7.28E-4 -1.60E-3
PERE = Use of renewable primary energy excluding renewable primary energy resources used as raw materials; PERM = Use of
renewable primary energy resources used as raw materials; PERT = Total use of renewable primary energy resources; PENRE = Use of
non-renewable primary energy excluding non-renewable primary energy resources used as raw materials; PENRM = Use of non-
Caption
renewable primary energy resources used as raw materials; PENRT = Total use of non-renewable primary energy resources; SM = Use
of secondary material; RSF = Use of renewable secondary fuels; NRSF = Use of non-renewable secondary fuels; FW = Use of net fresh
water
RESULTS OF THE LCA – WASTE CATEGORIES AND OUTPUT FLOWS according to EN 15804+A1:
1 m² 30mm PROMATECT®-L500
Parameter Unit A1 A2 A3 A4 A5 B1 B2 B6 B7 C1 C2 C3 C4 D
HWD [kg] 1.11E-3 1.48E-10 4.77E-8 7.15E-11 5.53E-5 0.00E+0 0.00E+0 0.00E+0 0.00E+0 0.00E+0 3.42E-11 0.00E+0 3.13E-10 -1.62E-9
NHWD [kg] 3.51E-1 4.92E-4 1.07E+0 2.13E-4 8.19E-1 0.00E+0 0.00E+0 0.00E+0 0.00E+0 0.00E+0 1.02E-4 0.00E+0 1.47E+1 -3.39E-3
RWD [kg] 2.34E-3 5.66E-6 1.14E-3 2.46E-6 1.91E-4 0.00E+0 0.00E+0 0.00E+0 0.00E+0 0.00E+0 1.18E-6 0.00E+0 3.09E-5 -5.26E-4
CRU [kg] 0.00E+0 0.00E+0 0.00E+0 0.00E+0 0.00E+0 0.00E+0 0.00E+0 0.00E+0 0.00E+0 0.00E+0 0.00E+0 0.00E+0 0.00E+0 0.00E+0
MFR [kg] 0.00E+0 0.00E+0 1.44E-1 0.00E+0 7.20E-3 0.00E+0 0.00E+0 0.00E+0 0.00E+0 0.00E+0 0.00E+0 0.00E+0 0.00E+0 0.00E+0
MER [kg] 0.00E+0 0.00E+0 0.00E+0 0.00E+0 0.00E+0 0.00E+0 0.00E+0 0.00E+0 0.00E+0 0.00E+0 0.00E+0 0.00E+0 0.00E+0 0.00E+0
EEE [MJ] 0.00E+0 0.00E+0 1.98E-4 0.00E+0 1.79E+0 0.00E+0 0.00E+0 0.00E+0 0.00E+0 0.00E+0 0.00E+0 0.00E+0 0.00E+0 0.00E+0
EET [MJ] 0.00E+0 0.00E+0 4.56E-4 0.00E+0 3.23E+0 0.00E+0 0.00E+0 0.00E+0 0.00E+0 0.00E+0 0.00E+0 0.00E+0 0.00E+0 0.00E+0
HWD = Hazardous waste disposed; NHWD = Non-hazardous waste disposed; RWD = Radioactive waste disposed; CRU = Components
Caption for re-use; MFR = Materials for recycling; MER = Materials for energy recovery; EEE = Exported electrical energy; EET = Exported
thermal energy
6. LCA: Interpretation
The following graph provides information on the
relative contributions of the declared modules to
various environmental impact categories.
For the raw materials, very important impacts (>25 %)
It can be seen that the main contributions to the impact are coming from the lime (GWP, ODP, EP, POCP,
categories are coming from the production stage, more ADPF), the fibres (AP, ADPE) and the silica sand
specifically from the raw material and the (ADPE).
manufacturing. The transport of the raw materials, the For the manufacturing, impacts are mainly coming
transport of the product to the building site, the waste from the energy required for the production process for
treatment of the packaging and the end-of-life modules heating the reactors to form the calcium silicate and for
only contribute to a minor extent. drying the boards.
7. Requisite evidence
Name Value Unit
Total VOC after 28d (C-C16)
13 µg/m³
7.1 Radioactivity measurements Limit : 1000
Radioactivity measurements confirm that no other R after 28d (c/NIK) 0.032 -
gamma emitters than those originating from natural Sum of VVOC after 28d (<n-C6) < 5 µ g /m³
radiation sources are contained. The measured Sum of SVOC after 28d (>n-C16)
<5 µg/m³
radioactivity levels do not exceed the activity Limit : 100
concentration indices as specified by Article 3 Sum of cancerogenic
<1 µg/m³
(Radiation Protection 112) for building products Limit : 1
following the Council Formaldehyd
Directive 96/29. Activity concentration index ≤ 2. Limit : 120 <5 µg/m³
Date: 2 December 2011 Acetaldehyd <5 µg/m³
Measuring agency: SCK.CEN Laboratory for
Date: 25 September 2008
Gammaspectrometry, Mol, Belgium
Measuring agency: Eurofins Product Testing A/S,
Protocol: Activity concentration index (ACI)
Galten, Denmark
Report number: 765393F
7.2 VOC emissions
VOC measurements confirmed compliance with the
requirements of DIBt DIBt-communication 4/2004 in
combination with the NIK values from AgBB (March
2008) for use in the indoor environment. (values in the
table below having "<" means that the measurements
were below the quantification limit)
8 Environmental Product Declaration Etex Building Performance NV – PROMATECT®-L500
8. References
Standards
BBSR
EN 826 BBSR table "Service lives of components for life cycle
EN 826: 1996: Thermal insulating products for building assessment according to Bewertungssystem
applications - Determination of compression behaviour Nachhaltiges Bauen (BNB)" Sustainable Building
Information Portal by the Federal Ministry of Transport,
EN 1607 Building and Urban Affairs (Bundesinstitut für Bau-
EN 1607: 1996: Thermal insulating products for ,Stadt-und Raumforschung, BBSR).
building applications - Determination of tensile strength (https://www.nachhaltigesbauen.de/baustoff-
perpendicular to faces undgebaeudedaten/
nutzungsdauern-von-bauteilen.html)
EN 1608
EN 1608: 1996: Thermal insulating products for Candidate list
building applications - Determination of tensile strength Candidate List of substances of very high concern for
parallel to faces Authorisation, published on ECHA website, latest
version 19.01.2021. (https://echa.europa.eu/candidate-
EN 12467 list-table)
EN 12467: 2004: Fibre-cement flat sheets - Product
specification and test methods CPR
Construction Products Regulation, Regulation (EU) No
EN 12667 305/2011 of the European Parliament and of the
EN 12667: 2001: Thermal performance of building Council of 9 March 2011 laying down harmonized
materials and products- Determination of thermal conditions for the marketing of construction products
resistance by means of guarded hot plate and heat and repealing Council Directive 89/106/ EEC Text with
flow meter methods. Products of high and medium EEA relevance.
thermal resistance.
DIBt-communication 4/2004
EN 13501-1 DIBt (Deutsches Institut für Bautechnik) approval
EN 13501-1:2018, Fire classification of construction guidelines for the health-related evaluation of indoor
products and building elements - Part 1: Classification construction products-2004
using data from reaction to fire tests.
Directive 96/29
EN 15804 Council Directive 96/29/Euratom of 13 May 1996 laying
EN 15804:2012+A2:2019, Sustainability of down basic safety standards for the protection of the
construction works — Environmental Product health of workers and the general public against the
Declarations — Core rules for the product category of dangers arising from ionising radiation
construction products.
European List of Waste
ISO 9001 2014/955/EU: Commission Decision of 18 December
UNI EN ISO 9001:2015 September 2015, Quality 2014 amending Decision 2000/532/EC on the list of
management systems - Requirements waste pursuant to Directive 2008/98/EC of the
European Parliament and of the Council.
ISO 12572 (http://data.europa.eu/eli/dec/2014/955/oj)
DIN EN ISO 12572:2001, Hygrothermal performance
of building materials and products - Determination of ETA 06/0218
water vapour transmission properties - Cup method European technical approval of PROMATECT®-L500
fire protective board
ISO 14001
UNI EN ISO 14001:2015, Environmental management Eurofins Product Testing A/S
systems - Requirements with guidance for use. Eurofins Product Testing A/S, Smedeskovvej 38, 8464
Galten, Denmark. Report number: 765393F; 2008.
ISO 14025
DIN EN ISO 14025:2011-10, Environmental labels and GaBi
declarations — Type III environmental declarations — GaBi Software System and Database for Life Cycle
Principles and procedures. Engineering, 1992-2021, Sphera Solutions GmbH,
Leinfelden-Echterdingen, with acknowledgement of
ISO 45001 LBP University of Stuttgart, program version GaBi 10;
ISO 45001:2018, Occupational health and safety database version 2021.1.
management systems — Requirements with guidance
for use GaBi documentation
GaBi dataset documentation for the software system
Further References and databases, LBP, University of Stuttgart and
Sphera Solutions GmbH, Leinfelden-Echterdingen,
AgBB 2021.
Ausschuss zur gesundheitlichen Bewertung von (http://www.gabi-software.com/support/gabi/gabi-
Bauprodukten, AgBB (eng. German Committee for database-2021-lci-documentation/)
health-related evaluation of building products.
9 Environmental Product Declaration Etex Building Performance NV – PROMATECT®-L500
IBU 2021 insulating materials, version 1.6, 2017 www.bau-
Institut Bauen und Umwelt e.V.: General Programme umwelt.de
Instructions for the Preparation of EPDs at the Institut
Bauen und Umwelt e.V. Version 2.0, Berlin: Institut REACH Regulation
Bauen und Umwelt e.V., 2021. Regulation (EU) No 1907/2006 of the European
(http://www.ibu-epd) Parliament and of the Council of 18 December 2006
concerning the Registration, Evaluation, Authorisation
Ordinance on Biocide Products and Restriction of Chemicals (REACH), establishing a
Regulation (EU) No 528/2012 of the European European Chemicals Agency, amending Directive
Parliament and of the Council of 22 May 2012 1999/45/EC and repealing Council Regulation (EEC)
concerning the making available on the market and No 793/93 and Commission
use of biocidal products. Regulation (EC) No 1488/94 as well as Council
Directive 76/769/EEC and Commission Directives
PCR Part A 91/155/EEC, 93/67/EEC, 93/105/EC and 2000/21/EC.
PCR Part A: Calculation rules for the Life Cycle
Assessment and Requirements on the Background SCK CEN Laboratory
Report according to EN 15 804+A2:2019, Version 1.0, Belgian Nuclear Research Centre in Mol.
Institut Bauen und Umwelt e.V., 2020.
PCR Part B
Product Category Rules for Building Products, Part B:
Requirements on the EPD for Calcium silicate
10 Environmental Product Declaration Etex Building Performance NV – PROMATECT®-L500
Publisher
Institut Bauen und Umwelt e.V. Tel +49 (0)30 3087748- 0
Panoramastr. 1 Fax +49 (0)30 3087748- 29
10178 Berlin Mail info@ibu-epd.com
Germany Web www.ibu-epd.com
Programme holder
Institut Bauen und Umwelt e.V. Tel +49 (0)30 - 3087748- 0
Panoramastr 1 Fax +49 (0)30 – 3087748 - 29
10178 Berlin Mail info@ibu-epd.com
Germany Web www.ibu-epd.com
Author of the Life Cycle
Assessment Tel +32 (0)15 71 82 83
Peggy Van De Velde Fax +32 (0)15 71 82 29
Bormstraat 24 Mail
2830 Tisselt peggy.vandevelde@etexgroup.c
Belgium om
Web www.etexgroup.com
Owner of the Declaration
Etex Building Performance Tel +32 2 778 12 11
International Fax +32 2 778 12 12
Rue Marcel Demonque 500 r Mail info@etexgroup.com
84915 Avignon Cedex 9 Web http://www.etexgroup.com
France
