ENVIRONMENTAL PRODUCT DECLARATION
as per ISO 14025 and EN 15804+A2
Owner of the Declaration voestalpine AG
Publisher Institut Bauen und Umwelt e.V. (IBU)
Programme holder Institut Bauen und Umwelt e.V. (IBU)
Declaration number EPD-VOE-20230108-IBC2-EN
Issue date 09.05.2023
Valid to 08.05.2028
Drawn Wire - Prestressing Wire and Strand
voestalpine Wire Austria GmbH
www.ibu-epd.com | https://epd-online.com
1. General Information
voestalpine Wire Austria GmbH Drawn Wire - Prestressing Wire and Strand
Programme holder Owner of the declaration
IBU – Institut Bauen und Umwelt e.V. voestalpine AG
Hegelplatz 1 voestalpine-Straße 3
10117 Berlin 4020 Linz
Germany Austria
Declaration number Declared product / declared unit
EPD-VOE-20230108-IBC2-EN 1 tonne of prestressing steel
This declaration is based on the product category rules: Scope:
Structural steels, 01.08.2021 This EPD is based on a declared unit of 1 metric tonne of average
(PCR checked and approved by the SVR) voestalpine prestressing steel produced at the production site in Bruck a.d.
Mur (Austria).
The owner of the declaration shall be liable for the underlying information
Issue date and evidence; the IBU shall not be liable with respect to manufacturer
information, life cycle assessment data and evidences.
09.05.2023
The EPD was created according to the specifications of EN 15804+A2. In
the following, the standard will be simplified as EN 15804.
Valid to
08.05.2028 Verification
The standard EN 15804 serves as the core PCR
Independent verification of the declaration and data according to ISO
14025:2011
internally X externally
Dipl.-Ing. Hans Peters
(Chairman of Institut Bauen und Umwelt e.V.)
Florian Pronold Prof. Dr. Birgit Grahl,
(Managing Director Institut Bauen und Umwelt e.V.) (Independent verifier)
1 Environmental Product Declaration - voestalpine Wire Austria GmbH - Drawn Wire - Prestressing Wire and Strand
2. Product
2.1 Product description/Product definition
Prestressing wires and strands are used for reinforcing
concrete structures, such as large-span bridges, rock-soil
anchoring solutions, multi-storey industrial buildings, stadiums,
mines, sleepers etc.
The prestressing wires are produced according to FprEN
10138-2:2009 besides many other standards and
homologations. Diameters range from 5.0 up to 10.5 mm.
Our 7-wire prestressing strands are supplied with cross-
sectional areas ranging from 139 to 165 mm², depending on
customer requirements, and with smooth or compacted surface.
Compacted prestressing strands have a cross-sectional area of
165 mm². All strands exhibit very low relaxation. They are
produced according to FprEN 10138-3:2009 besides other The prestressing strands are produced according to FprEN
standards and homologations. Diameters range from 15.2 to 10138-3:2009 besides other standards and homologations.
15.7 mm for bare and compacted strands.
Diameter and tensile strength class of Prestressing Strands:
voestalpine Wire Technology also manufactures a variety of
strand types with corrosion protection. The strands can be
oiled, galvanized and additionally greased or waxed and PE-
coated. Due to their excellent properties, these products are
suitable for a wide variety of uses.
The prestressing products are manufactured under ideal
processing conditions to ensure they meet the most demanding
quality standards.
• Continuous quality inspections and many special testing Performance data of the product with respect to its
options characteristics in accordance with the relevant technical
• End-to-end traceability of all production and test provision (no CE-marking).
parameters
2.4 Delivery status
• Greatest possible flexibility as the result of an integrated
The prestressing wires can be delivered in coils, bars, threaded
production chain
bars or threaded hairpins.
• Strict adherence to schedules, and partnerships with our
The prestressing strands can be delivered in coils or on
customers
wooden reels.
• Technical and sales service
2.5 Base materials/Ancillary materials
For the use and application of the product the respective
Base materials:
national provisions at the place of use apply, in Germany for
The starting product for prestressing steel is hot-rolled wire,
example the building codes of the federal states and the
which is produced at the voestalpine Wire Rod Austria site. The
corresponding national specifications.
basic material for this is in turn crude steel, which consists of
2.2 Application about 85 % pig iron and about 15 % scrap.
Prestressing wires are mainly used for prestressing of concrete
The corrosion protection is given by oiling, galvanizing,
sleepers but can find their application also in prefabricated
greasing or waxing and PE-coating.
parts, beams, or reinforced tubes. Bare strands and PE-coated
strands for prestressed concrete are suitable for large-span and
The mass of zinc for galvanized strands is 190 –350 g/m².
large bays cast-in-place concrete floors, precast elements and
The minimum sheathing thickness of PE-coated strands is 1.25
beams and other special structures. As an additional
mm.
application, these strands can be used in wind tower
construction and anchoring systems. Galvanized and PE-
For our extrusion technology different HDPE-types like
coated strands mainly are used in stay-cable bridges.
HDPE80, HDPE100 or HDPE100+ can be used.
2.3 Technical Data
The prestressing wires are produced according to FprEN This product/article/at least one partial article contains
10138-2:2009 besides other standards and homologations. The substances listed in the candidate list (date: 16.1.2020)
technical data given for the products are generic literature data exceeding 0.1 percentage by mass: no.
for steel as described e.g. in Key to Steel. No product specific
test rules are applicable to the data given. This product/article/at least one partial article contains other
carcinogenic, mutagenic, reprotoxic (CMR) substances in
Diameter and tensile strength class of Prestressing Wires: categories 1A or 1B which are not on the candidate list,
exceeding 0.1 percentage by mass: no.
Biocide products were added to this construction product or it
has been treated with biocide products (this then concerns a
2 Environmental Product Declaration - voestalpine Wire Austria GmbH - Drawn Wire - Prestressing Wire and Strand
treated product as defined by the (EU) Ordinance on Biocide periodically inspected by the authorities as part of
Products No. 528/2012): no. environmental inspections.
2.6 Manufacture 2.8 Product processing/Installation
Manufacturing of prestressing strands voestalpine drawn wire can be processed using cold-forming
The starting process is the pickling process. During pickling methods, such as cold heading, spring coiling, etc.. Such
scale and rust from the surface of the wire rod coil are removed processing methods do not produce any emissions or other
by dipping into hydrochloric acid. After several other treatments harmful influences that emanate from the declared product.
like phosphate coating and borax coating the wire rod coil is
prepared for the next step cold drawing. 2.9 Packaging
The declared product is delivered as described in 2.4. The
On the drawing line, the single wire is drawn to the final packaging can consist of paper (coated), steel straps
diameter on a spool. Seven of these spools finally are lifted into (circumferential straps as well as axle hole straps) and
the skip strander, where a seven-wire prestressing strand is cardboard tubes and varies depending on the delivery. The
produced. The main process during stranding is the packaging can be completely recycled.
thermomechanical treatment (pulling and heating = stabilizing)
2.10 Condition of use
to finally get the special properties like low relaxation and good
ductility on a high tensile level. Prestressing wires and strands are well protected either in the
concrete structure or by using HDPE-pipes as an additional
In case of a galvanized strand the wire is pre-drawn and outer protection in case of stay-cable-bridges. Due to this fact,
galvanized in our hot dip galvanizing line. After galvanizing the changes in material composition or changes of environmentally
final drawing and the stranding remain the same. relevant inherent properties can be excluded.
2.11 Environment and health during use
In case of HDPE-coated strands, the smooth, compacted or
During the use of our prestressing products on site no danger
galvanized strands are greased or waxed and afterwards
for environment and health can occur, because of the dry and
HDPE-coated in our extrusion line. We can produce the coated
clean or well protected surface. Of course all relevant safety
strands from coil to coil either as reelless coils or on wooden
instructions on site have to be followed strictly.
reels.
2.12 Reference service life
Manufacturing of prestressing steel wires
The reference useful life depends on the type of application and
The starting process is the pickling process. During pickling
is usually between 15 and 50 years. Corrosive atmospheres
scale and rust from the surface of the wire rod coil are removed
have to be avoided to guarantee a full lifetime of functionality.
by dipping into hydrochloric acid. After several other treatments
like phosphate coating and borax coating the wire rod coil is 2.13 Extraordinary effects
prepared for the next step cold drawing. Fire
Not relevant.
On the combined drawing and stabilizing line, the single wire is
drawn to the final diameter either in coils or in bars. The main Water
process during drawing is the thermomechanical treatment No negative consequences for the environment are to be
(pulling and heating = stabilizing) to finally get the special expected under the influence of water.
properties like low relaxation and good ductility on a high
tensile level. Mechanical destruction
Unforeseen mechanical impact on the declared product has no
The wires in coils are directly sent to final customers, the wires negative consequences on the environment due to the plastic
in bars can be additionally bent and threaded or just only deformability of steel.
threaded at the end of the bars. Thus, all different types of
wires needed for sleeper production (bars, threaded bars, coils 2.14 Re-use phase
or threaded hairpins) can be provided. Wire from voestalpine can either be reused or recycled and
reintroduced into the steel industry as a secondary raw material
2.7 Environment and health during manufacturing
via recycling companies.
The voestalpine Wire Austria site is certified according to EMAS
III, ISO 9001, ISO 50001 and ISO 14001. As part of the 2.15 Disposal
environmental declarations required by EMAS, voestalpine The declared product can be fully used as a recycling raw
continuously publishes environmentally relevant data and facts material. The waste code according to the European Waste
about the site. Catalogue is: 17 04 05. The waste type is equivalent to the key
number 35103 according to the nationally applicable Waste
At the Bruck/Mur site, investments are constantly being made in Catalogue by-law.
the expansion of environmental protection measures in order to
be able to reduce emissions to air and water to a minimum. 2.16 Further information
Further information on the product is available on the website at
All operating facilities that have been approved in accordance https://www.voestalpine.com/wiretechnology/en/company/product-
with the environmental impact assessment procedure are also earch/Prestressing-Wire/
3. LCA: Calculation rules
Name Value Unit
3.1 Declared Unit
Declared unit 1 t
This environmental product declaration refers to a declared unit
of 1 tonne of average prestressing steel.
Density 7850 kg/m3
Declared unit
3 Environmental Product Declaration - voestalpine Wire Austria GmbH - Drawn Wire - Prestressing Wire and Strand
For the calculation of the declared average, input and assumptions from average data (when available) or with
production quantities for the entire calendar year 2018 were generic data and are documented accordingly. Only data with a
taken into account and broken down to the declared product contribution of less than 1 % were cut off. Ignoring such data is
group. The calculated results can thus be considered justified based on the irrelevance of the expected effect.
representative for the declared product portfolio of prestressing Processes, materials, or emissions known to make a significant
steel of voestalpine Wire Austria GmbH. contribution to the environmental effects of the products under
examination have not been neglected. All relevant data were
A linear correlation of the environmental impacts with the collected comprehensively. It is assumed that the data have
product weight is to be expected. Therefore, the conversion been completely recorded and the overall total of ignored input
from the declared unit to a specific product is possible using a flows do not amount to more than 5 % of total energy and mass
mass-specific scaling factor. flows.
Environmental impacts of machines, plant and infrastructure
3.2 System boundary were not included.
The life cycle assessment of average prestressing steel refers
to a cradle-to-gate analysis with modules (A1–A3 + C +D). 3.5 Background data
Subsequent life cycle phases are part of the analysis: This study uses generic background data for the evaluation of
upstream environmental impacts from GaBi-database 2021.1
Module A1–A3 | Production stage and is modelled in GaBi-software version 10.
The production stage includes the burdens of the production of
prestressing steel of voestalpine Wire Austria GmbH at the 3.6 Data quality
production site in Bruck a.d. Mur. Most of the used steel wire is The foreground data collected at voestalpine Wire Austria
provided by the voestalpine Wire Rod Austria from St. Peter GmbH are based on the quantities used and volumes produced
Freienstein. Thus, the upstream environmental impact of the annually. Process data were collected by voestalpine in the
steel supplied is represented by primary data of the respective course of reporting to official agencies. Data on material and
production site. Material and energy flows for the pickling, energy use originate from material-specific throughput
drawing, cold rolling and galvanizing are considered. Electricity measurements of various processes as well as from controlling.
at Bruck a. d. Mur is provided from 100 % renewable energy The technological, geographical and time-related
(emission factor GWP-total: 14 g CO -equivalents/kWh). representativeness of the data base was kept in mind when
2
selecting background data. Whenever specific data were
Thermal energy provision is based on natural gas. Module A1–
missing, either generic datasets or representative average data
A3 also includes the production of the packaging.
were used instead. The implemented GaBi background
datasets are not more than ten years old.
Module C1 | Deconstruction and demolition
It is assumed that the product is not connected with other
3.7 Period under review
materials and can therefore be dismantled. Associated efforts
Foreground data were collected in the 2018 production year,
are negligible, no environmental impacts from the
and the data are based on the volumes produced on an annual
deconstruction of the products are declared.
basis.
Module C2 | Transport 3.8 Geographic Representativeness
The transport to the disposal of the material is estimated
Land or region, in which the declared product system is
declaring a 50 km radius to the waste processing.
manufactured, used or handled at the end of the product´s
lifespan: Austria
Module C3 | Waste processing
Product flows that reach Module D for recycling leave the
product system in C3. Environmental impacts resulting from the 3.9 Allocation
grinding and sorting of steel scrap are not included due to the The primary data for the upstream production of the steel billets
negligible expected environmental impact. were allocated using the partitioning approach developed by
worldsteel 2014 for calculating life cycle inventories of co-
Module C4 | Landfilling products in steel production, which is in line with the provisions
Module C4 declares the environmental impacts incurred by of EN 15804. The so-called partitioning approach provides for
landfilling (5 % of the product). the allocation of environmental effects on the steelmaking
process and the emerging byproducts based on physical
Module D | Benefits and loads beyond the system relations. Material-inherent flow properties are, thus, taken into
boundary account.
The potential for substituting primary steel with a recycling
scenario (95 % of the product) is outlined in Module D. Economic allocation is not considered as referring byproducts
and co-products are not directly tradable goods. Furthermore,
3.3 Estimates and assumptions
long-term contracts for the sale of the byproducts exist, and the
All assumptions are verified through detailed documentation
negotiated prices are, therefore, not subject to market
and correspond to the best possible representation of reality
dynamics.
based on the available data. Regional applicability of the used
background data refers to average data under European or 3.10 Comparability
German conditions taken from the GaBi-database. German Basically, a comparison or an evaluation of EPD data is only
data were used for the Austrian market whenever European or possible if all the data sets to be compared were created
Austrian average data were not available. according to EN 15804 and the building context, respectively
the product-specific characteristics of performance, are taken
3.4 Cut-off criteria
into account. The GaBi background database was used to
All inputs and outputs for which data are available are included
calculate the LCA (GaBi 10; 2021.1).
in the LCA model. Data gaps are filled with conservative
4 Environmental Product Declaration - voestalpine Wire Austria GmbH - Drawn Wire - Prestressing Wire and Strand
4. LCA: Scenarios and additional technical information
The end-of-life scenario used in this LCA study is based on the
Characteristic product properties of biogenic carbon following assumptions and thus complies with the specifications
The declared product does not contain any biogenic carbon. published in ökobaudat 2022:
Information on describing the biogenic Carbon Content at End of life (C1–C4)
factory gate
Name Value Unit
Name ValueUnit
Collected separately waste type (steel) 1000 kg
Biogenic carbon content in accompanying kg
1.84 Recycling 95 % 950 kg
packaging C
Landfilling 5 % 50 kg
The carbon stored in the packaging was taken into account as
"CO -neutral". Thus the storage effect of the carbon bound in Reuse, recovery and/or recycling potentials (D), relevant
2
scenario information
the packaging is not included in the calculation but is
considered as emitted immediately. Name Value Unit
Net flow of steel scrap 882 kg
This scenario contains a recycling rate of 95 %. Since
voestalpine externally purchases scrap for steel production, this
is offset against the steel scrap for recycling (net flow).
Installation into the building (A5)
The end-of-life of the packaging materials is not declared in
Module A5.
Name Value Unit
Packaging (binding wire, packaging strips) 1.04 kg
Packaging (plastic) 0.03 kg
Packaging (cardboard) 0.0008 kg
Packaging (wood) 4.12 kg
5 Environmental Product Declaration - voestalpine Wire Austria GmbH - Drawn Wire - Prestressing Wire and Strand
5. LCA: Results
The following table contains the LCA results for a declared unit of 1 tonne of prestressing steel.
DESCRIPTION OF THE SYSTEM BOUNDARY (X = INCLUDED IN LCA; ND = MODULE OR INDICATOR NOT DECLARED; MNR =
MODULE NOT RELEVANT)
Benefits and
Construction loads beyond
Product stage Use stage End of life stage
process stage the system
boundaries
la ire ta m w a Ry lp p u s tro p s n a rT g n iru tc a fu n a M e h t m o rf tro p s n a rTe tis e h t o t e ta g y lb m e s s A e s U e c n a n e tn ia M ria p e R tn e m e c a lp e R tn e m h s ib ru fe R y g re n e la n o ita re p Oe s u re ta w la n o ita re p Oe s u n o itc u rts n o c -e Dn o itilo m e d tro p s n a rT g n is s e c o rp e ts a W la s o p s iD -e s u e R-y re v o c e R-g n ilc y c e Rla itn e to p
A1 A2 A3 A4 A5 B1 B2 B3 B4 B5 B6 B7 C1 C2 C3 C4 D
X X X MND MND MND MND MNR MNR MNR MND MND X X X X X
RESULTS OF THE LCA - ENVIRONMENTAL IMPACT according to EN 15804+A2: 1 tonne prestressing steel
Parameter Unit A1-A3 C1 C2 C3 C4 D
Global Warming Potential total (GWP-total) kg CO 2 eq 2.91E+03 0 3.02E+00 0 2.42E+00 -1.5E+03
Global Warming Potential fossil fuels (GWP-fossil) kg CO 2 eq 2.9E+03 0 3E+00 0 2.44E+00 -1.49E+03
Global Warming Potential biogenic (GWP-biogenic) kg CO 2 eq 1.65E+01 0 -3.56E-03 0 -2.5E-02 -9.68E-01
Global Warming Potential luluc (GWP-luluc) kg CO 2 eq 1.06E+00 0 2.44E-02 0 2.44E-03 2.16E-01
Depletion potential of the stratospheric ozone layer (ODP) kg CFC11 eq 2.18E-11 0 5.9E-16 0 5.77E-15 -2.49E-12
Acidification potential of land and water (AP) mol H+ eq 9.09E+00 0 9.92E-03 0 7.78E-03 -2.68E+00
Eutrophication potential aquatic freshwater (EP-freshwater) kg P eq 1.52E-02 0 8.88E-06 0 1.86E-06 -3.06E-04
Eutrophication potential aquatic marine (EP-marine) kg N eq 2.19E+00 0 4.55E-03 0 1.93E-03 -4E-01
Eutrophication potential terrestrial (EP-terrestrial) mol N eq 2.33E+01 0 5.08E-02 0 2.12E-02 -3.9E+00
Formation potential of tropospheric ozone photochemical oxidants kg NMVOC
7.31E+00 0 8.94E-03 0 6.08E-03 -2.05E+00
(POCP) eq
Abiotic depletion potential for non fossil resources (ADPE) kg Sb eq 4.58E-03 0 2.65E-07 0 1.68E-07 -3.25E-03
Abiotic depletion potential for fossil resources (ADPF) MJ 2.63E+04 0 3.98E+01 0 3.56E+01 -1.3E+04
m3 world eq
Water use (WDP) 5.23E+02 0 2.77E-02 0 -2.89E-02 -2.93E+02
deprived
RESULTS OF THE LCA - INDICATORS TO DESCRIBE RESOURCE USE according to EN 15804+A2: 1 tonne prestressing steel
Parameter Unit A1-A3 C1 C2 C3 C4 D
Renewable primary energy as energy carrier (PERE) MJ 3.19E+03 0 2.29E+00 0 2.57E+00 1.2E+03
Renewable primary energy resources as material utilization
MJ 6.81E+01 0 0 0 0 0
(PERM)
Total use of renewable primary energy resources (PERT) MJ 3.26E+03 0 2.29E+00 0 2.57E+00 1.2E+03
Non renewable primary energy as energy carrier (PENRE) MJ 2.64E+04 0 4E+01 0 3.56E+01 -1.3E+04
Non renewable primary energy as material utilization (PENRM) MJ 1.16E+00 0 0 0 0 0
Total use of non renewable primary energy resources (PENRT) MJ 2.64E+04 0 4E+01 0 3.56E+01 -1.3E+04
Use of secondary material (SM) kg 1.17E+02 0 0 0 0 8.82E+02
Use of renewable secondary fuels (RSF) MJ 0 0 0 0 0 0
Use of non renewable secondary fuels (NRSF) MJ 0 0 0 0 0 0
Use of net fresh water (FW) m3 1.62E+01 0 2.62E-03 0 3.67E-04 -6.59E+00
RESULTS OF THE LCA – WASTE CATEGORIES AND OUTPUT FLOWS according to EN 15804+A2:
1 tonne prestressing steel
Parameter Unit A1-A3 C1 C2 C3 C4 D
Hazardous waste disposed (HWD) kg 3.91E-04 0 2.11E-09 0 6.3E-09 3.63E-06
Non hazardous waste disposed (NHWD) kg 6.6E+01 0 6.27E-03 0 5.01E+01 1.56E+02
Radioactive waste disposed (RWD) kg 1.21E-01 0 7.25E-05 0 4.05E-04 4.71E-04
Components for re-use (CRU) kg 0 0 0 0 0 0
Materials for recycling (MFR) kg 0 0 0 9.5E+02 0 0
Materials for energy recovery (MER) kg 0 0 0 0 0 0
Exported electrical energy (EEE) MJ 0 0 0 0 0 0
Exported thermal energy (EET) MJ 0 0 0 0 0 0
RESULTS OF THE LCA – additional impact categories according to EN 15804+A2-optional:
1 tonne prestressing steel
Parameter Unit A1-A3 C1 C2 C3 C4 D
Disease
Incidence of disease due to PM emissions (PM) ND ND ND ND ND ND
incidence
Human exposure efficiency relative to U235 (IR) kBq U235 eq ND ND ND ND ND ND
Comparative toxic unit for ecosystems (ETP-fw) CTUe ND ND ND ND ND ND
6 Environmental Product Declaration - voestalpine Wire Austria GmbH - Drawn Wire - Prestressing Wire and Strand
Comparative toxic unit for humans (carcinogenic) (HTP-c) CTUh ND ND ND ND ND ND
Comparative toxic unit for humans (noncarcinogenic) (HTP-nc) CTUh ND ND ND ND ND ND
Soil quality index (SQP) SQP ND ND ND ND ND ND
The additional and optional impact categories according to EN 15804+A2 are notdeclared, as the uncertainty of these indicators is to
be classified as high.
Disclaimer 1 – for the indicator potential human exposure efficiency relative to U235:
This impact category deals mainly with the eventual impact of low dose ionizing radiation on human health of the nuclear fuel cycle. It
does not consider effects due to possible nuclear accidents, occupational exposure nor radioactive waste disposal in underground
facilities. Potential ionizing radiation from the soil, from radon and from some construction materials is also not measured by this
indicator.
Disclaimer 2 – for the indicators abiotic depletion potential for non-fossil resources, abiotic depletion potential for fossil resources, water
(user) deprivation potential, deprivation weighted water consumption, eutrophication fraction of nutrients reaching freshwater end
compartment, potential comparative toxic unit for humans cancerogenic, potential comparative toxic unit for humans not cancerogenic,
potential soil quality index:
The results of this environmental impact indicator shall be used with care as the uncertainties on these results are high or as there is
limited experience with the indicator.
6. LCA: Interpretation
The following interpretation contains a summary of the LCA steel.
results referenced to a declared unit of 1 tonne of prestressing
A comparison of the individual lifecycle phases results in a clear
dominance of the production phase (modules A1–A3). The Most of the potential environmental impacts of the production
environmental effects in the production phase are mainly phase (module A1–A3) of the prestressing steel can be traced
dominated by the direct process emissions of billet production. back to the upstream supply of the wire rod. The production of
prestressing steel at the production site at Bruck contributes
As a result of product recyclability, the material removed at the app. 5 % to global warming potential.
end of life can substitute primary steel. According to the set
method, the first step is to saturate the secondary material used A linear correlation of the environmental impacts with the
in module A with material from module C. The excess amount product weight is to be expected. Therefore, the conversion
from module C ('net flow') can substitute primary steel and from the declared unit to a specific product is possible using a
leads to corresponding substitution potentials in module D. mass-specific scaling factor.
The environmental impact of the transport of the products to All primary data were specifically broken down to the declared
recycling (C2) as well as landfilling of the losses at the end of product group. As a result, the representativity of the results for
life (C4) represents a minor contribution to the overall the declared product group is to be expected as high.
environmental impact of the product.
7 Environmental Product Declaration - voestalpine Wire Austria GmbH - Drawn Wire - Prestressing Wire and Strand
7. Requisite evidence
Not relevant for this EPD.
8. References
Standards Guidance on classification of waste according to EWC Stat
categories. Supplement to the Manual for the Implementation of
EN 15804 the Regulation (EC) No 2150/2002 on Waste Statistics.
DIN EN 15804:2012+A2:2019+AC:2021, Sustainability of Commission of the European Communities, EUROSTAT.
construction works - Environmental product declarations - Core
rules for the product category of construction products. GaBi
GaBi 10, Software System and Database for Life Cycle
FprEN 10138-2 Engineering. DB 2021.1. Sphera, 1992-2021. Available in:
FprEN 10138-2:2009, Prestressing steels – Part 2: Wire. http://documentation.gabisoftware.com
FprEN 10138-3 IBU 2021
FprEN 10138-3:2009, Prestressing steels – Part 3: Strand. Institut Bauen und Umwelt e.V.: General guidance for the EPD
program of the Institut Bauen und Umwelt e.V.. (IBU). Version
ISO 9001 2.0, Berlin: Institut Bauen und Umwelt e.V., 2021.
ISO 9001:2015, Quality management systems – Requirements. www.ibu-epd.com
ISO 14001 Key to Steel
ISO 14001:2015, Environmental management systems – Key to Steel (Stahlschlüssel) 2019, 25. edition, 2023, Verlag
Requirements with guidance for use. Stahlschlüssel Wegst GmbH, Germany.
ISO 14025 ökobaudat 2022
DIN EN ISO 14025:2011-10, Environmental labels and ökobaudat 2022. EN 15804 and BNB compliant data for over
declarations - Type III environmental declarations - Principles 700 building products.
and procedures.
Ordinance on Biocide Products
ISO 14044 Regulation (EU) No 528/2012 of the European Parliament and
DIN EN ISO 14044:2006-10, Environmental management - Life of the Council of 22 May 2012 concerning the making available
cycle assessment - equirements and guidance. on the market and use of biocidal products.
ISO 50001 PCR Part A
ISO 50001:2018, Energy Management Systems. Product category rules for building-related products and
services. Part A: Calculation rules for life cycle assessment and
Further references project report requirements according to EN 15804+A2:2019.
Version 1.3. Berlin: Institut Bauen und Umwelt e.V.. (ed.), 2022.
Candidate list
Candidate List of Substances of Very High Concern (ECHA PCR: Structural steels
Candidate List) of 16.01.2020, published in accordance with Product category rules for building-related products and
Article 59 (10) of the REACH Regulation Helsinki: European services. Part B: Requirements for the EPD for structural steels.
Chemicals Agency. Version v0. Berlin: Institut Bauen und Umwelt e.V., 08.03.2023.
EMAS III worldsteel 2014
Regulation (EC) No 1221/2009 of the European parliament and World Steel Association, February 14, 2014: A methodology to
of the council of 25 November 2009 on the voluntary determine the LCI of steel industry co-products.
participation by organisations in a Community eco-management
and audit scheme (EMAS), repealing Regulation (EC) No worldsteel 2019
761/2001 and Commission Decisions 2001/681/EC and World Steel Association, 2019: Life cycle inventory
2006/193/EC. methodology report.
European Waste Catalogue
8 Environmental Product Declaration - voestalpine Wire Austria GmbH - Drawn Wire - Prestressing Wire and Strand
Publisher
Institut Bauen und Umwelt e.V. +49 (0)30 3087748- 0
Hegelplatz 1 info@ibu-epd.com
10117 Berlin www.ibu-epd.com
Germany
Programme holder
Institut Bauen und Umwelt e.V. +49 (0)30 3087748- 0
Hegelplatz 1 info@ibu-epd.com
10117 Berlin www.ibu-epd.com
Germany
Author of the Life Cycle Assessment
Daxner & Merl GmbH +43 676 849477826
Schleifmühlgasse 13/24 office@daxner-merl.com
1040 Wien www.daxner-merl.com
Austria
Owner of the Declaration
voestalpine AG +43/50304/15-0
voestalpine-Straße 3 info@voestalpine.com
4020 Linz www.voestalpine.com
Austria
9 Environmental Product Declaration - voestalpine Wire Austria GmbH - Drawn Wire - Prestressing Wire and Strand
