ENVIRONMENTAL PRODUCT DECLARATION
as per ISO 14025 and EN 15804+A2
Owner of the Declaration HALTON FOODSERVICE
Publisher Institut Bauen und Umwelt e.V. (IBU)
Programme holder Institut Bauen und Umwelt e.V. (IBU)
Declaration number EPD-HAL-20240075-IBA1-EN
Issue date 27/08/2024
Valid to 26/08/2029
UVI/F MARVEL – Demand Controlled Kitchen Ventilation
HALTON FOOD SERVICE
www.ibu-epd.com | https://epd-online.com
1. General Information
HALTON FOOD SERVICE UVI/F MARVEL – Demand Controlled Kitchen
Ventilation
Programme holder Owner of the declaration
IBU – Institut Bauen und Umwelt e.V. HALTON FOODSERVICE
Hegelplatz 1 Zone Technoparc Futura CS 80102
10117 Berlin 62402 BETHUNE Cedex
Germany France
Declaration number Declared product / declared unit
EPD-HAL-20240075-IBA1-EN 1 linear metre of UVI/F MARVEL hood, used to extract heat and cooking
steam for 365 days a year, for 8 hours a day, for 15 years
This declaration is based on the product category rules: Scope:
Ventilation systems for commercial kitchens, 24/01/2024 This document refers to UVI/F MARVEL hood produced by HALTON
(PCR checked and approved by the SVR) FOODSERVICE in France. This EPD represents the declaration of a
specific product UVI/F MARVEL Hood, with the declared unit of 1 linear
metre of hood, used to extract heat and cooking steam for 365 days a
Issue date year, for 8 hours a day, for 15 years.
The data collection for the ecological assessment occurred plant specific
27/08/2024
with current annual data. Consequently, the Life Cycle Assessment is
representative for this product.
The owner of the declaration shall be liable for the underlying information
Valid to
and evidence; the IBU shall not be liable with respect to manufacturer
26/08/2029 information, life cycle assessment data and evidences.
The EPD was created according to the specifications of EN 15804+A2. In
the following, the standard will be simplified as EN 15804.
Verification
The standard EN 15804 serves as the core PCR
Independent verification of the declaration and data according to ISO
14025:2011
internally X externally
Dipl.-Ing. Hans Peters
(Chairman of Institut Bauen und Umwelt e.V.)
Florian Pronold Dr. Matthew Fishwick,
(Managing Director Institut Bauen und Umwelt e.V.) (Independent verifier)
1 Environmental Product Declaration - HALTON FOOD SERVICE - UVI/F MARVEL – Demand Controlled Kitchen Ventilation
2. Product
Products No. 528/2012): no.
2.1 Product description/Product definition
The hood equipped with the MARVEL technology (MRV) can 2.6 Manufacture
adjust its airflow in real time to reduce airflow as much as Manufacturing and packaging of the UVI/F MARVEL hood at
possible. The product is manufactured from steel, electronics, the production site. In this case, manufacturing mainly refers to
aluminium, plastic. the assembling, configuring, and testing of the hoods from pre-
made parts. The assessment covers the electricity, LPG
The Capture Jet™ technology (UVI/F) is related to the consumption for forklifts and water use needed during the
association of two sets of nozzles supplied with an extremely production process. The electricity is modelled as site-specific
low supply air volume (a maximum of 30 m³/h/m of hood). energy mixes provided by local energy companies.The waste
These nozzles fit to the lower part of the hood front as well as streams from the manufacturing site include, wastewater, wood
the sides, encircling the perimeter of the covered cooking waste, cardboard, plastic and metal scrap (stainless steel and
areas. The horizontal nozzles increase the push/pull of the galvanised steel sheets).
thermal plume and smoke from the lower part of the hood front Any production waste generated is disposed of according by
due to the Venturi effect. It provides an assist to push vapours Halton's waste contractor.
back towards the filters. For the placing on the market of the
product in the European Union/European Free Trade 2.7 Environment and health during manufacturing
Association (EU/EFTA) (with the exception of Switzerland) Workplace and emission limits are regularly monitored and are
Regulation (EU) No. 305/2011 (CPR) applies. The product far below the prescribed limits.
needs a declaration of performance taking into consideration
2.8 Product processing/Installation
EN and the CE-marking.
The hood is installed in about 10 hours by 2 employees. The
For the application and use the respective national provisions hood is fixed by hand to the ceiling with the help of a lifter and
apply. some fixation devices.
2.2 Application 2.9 Packaging
The UVI/F MARVEL hood is used for professional kitchens. For product protection the hoods are individually packed in a
They can be installed above the cooking appliances and is cardboard box. All packaged products are wrapped with (low
used to remove fumes, odors, heat, humidity, and any airborne density polyethylene) PEBD/LDPE film on a wood pallet.
grease from the environment.
2.10 Condition of use
Different Halton sensors (Such as Thermal Imaging Matrix, Air
To ensure the longevity of the product, a weekly cleaning (using
temperature, and Indoor Environment Quality) detect the start
water with 1.5% soap) and annual check-up on different hood
of cooking, which then starts the hood.
parameters (Capture jets state, lighting state, state and number
As cooking activity intensifies, airflow and extraction rates
of filters, k factor, exhaust rates in intake rates) are
increase to extract heat and cooking steam.
recommended.
2.3 Technical Data
2.11 Environment and health during use
The technical properties are project-dependent (Airflow range).
The products do not emit any contaminants or substances that
The dimensions of the reference product is specified in the
are harmful to the environment or health during the use phase.
table below.
2.12 Reference service life
The service life is validated if the hood is installed following the
Constructional Data installation procedure. Reference service life for the cooker
Name Value Unit hoods is assumed 15 years.The reference service life is based
on the empirical value for the hoods when used in accordance
Length 1000 mm
with the care instructions.
Width 1400 mm
Height 500 mm 2.13 Extraordinary effects
Weight 134.5 kg Fire
power consumption (operation) 519 W The products are not classified as building materials (building
products) and are not subject to DIN 4102 and EN 13501-1.
Performance data of the product with respect to its Water
characteristics in accordance with the relevant technical No water-hazardous, toxic substances are washed-out to the
provision (no CE-marking). environment and water.
2.4 Delivery status
Mechanical destruction
The products vary in size as they are not catalogue products.
There are no relevant environmental impacts associated with
mechanical destruction.
2.5 Base materials/Ancillary materials
This product/article/at least one partial article contains other 2.14 Re-use phase
Carcinogenic, mutagenic, reprotoxic (CMR) substances in
The UVI/F MARVEL are not taken back by the manufacturer for
categories 1A or 1B which are not on the candidate list,
the purpose of reuse. Users can disassemble the products
exceeding 0.1 percentage by mass: no.
repeatedly within the reference utilization period and reuse it
elsewhere.
Biocide products were added to this construction product or it
has been treated with biocide products (this then concerns a 2.15 Disposal
treated product as defined by the (EU) Ordinance on Biocide
2 Environmental Product Declaration - HALTON FOOD SERVICE - UVI/F MARVEL – Demand Controlled Kitchen Ventilation
Disassembly of the products consists of the same steps as
assembly, in reverse order. The product falls under the Waste 2.16 Further information
from Electrical and Electronic Equipment (WEEE). Additional information about our products can be found on
Halton-website: www.halton.com.
3. LCA: Calculation rules
Module B2:
3.1 Declared Unit - a weekly cleaning with 5L of water containing 1.5% soap.
The declared unit is: '1 linear metre of hood, used to extract - annual check-up by a technician on different hood parameters
heat and cooking (Capture jets state, lighting state, filters (state and number), k
steam for 365 days a year, for 8 hours a day, for 15 years'. factor, exhaust rates in intake rates) modelled with
Declared unit transportation of one technician in light commercial vehicle
(100km). The number of check-ups depends on the hood
Name Value Unit
model.
Declared unit 1 rm
- 2 UV light replacements during the reference life service.
Mass per Unit 134.5 kg - End-of-life treatment of 2 UV light tubes during SLR with
linear density 134.5 kg/rm transportation included
Other declared units are allowed if the conversion is shown
Module B6 et B7
transparently.
The hood is designed for heavy duty industrial usage. To reflect
the most average scenario the hood will be functioning 8 hours
3.2 System boundary a days 7 days a week. Electricity (B6) is required to use the
products.
This representative EPD follows the EPD type "cradle to grave".
The following life cycle modules are declared:
Modules C1-C4
Modules A1-A3
The module includes the environmental impacts for dismantling
The product stage begins with considering the production of the
of the products and the treatment of the UVI/F MARVEL hood
necessary raw materials (metals, electronics, packaging
waste until the end-of-waste status (EoW) is reached, including
materials), including all corresponding upstream chains and the
the associated transports at the end of the product life
actual procurement transports.
cycle.The product is assumed to be removed manually at the
Furthermore, the entire manufacturing phase was mapped,
same time as the building is demolished. No scenario has been
including the treatment of production waste until the end-of
developed for stage C1.
waste status (EoW) was reached.
The hood and the ceiling beam are removed separately.
Module A4
Dismantling of product components at recycling facility. Based
The transport model considers a construction site in Europe.
on the material, components are either recycled, incinerated, or
The scenario for the distribution stage considers a average
landfilled depending on the material.
distance by truck to serve the entire European area from the
Halton's plant. The quantity transported corresponds to the
Stage C3 represents the impact of a conventional scrap
transport of products and their packaging to the construction
processing site, with sorting, shearing, shredding, separation.
site.
Module D
Module A5
Identification of the benefits and costs of the product outside
The hood is delivered at the right size on the installation site. It
the system boundary.
is installed in about 10 hours by 2 employees. The hood is fixed
Recycling of metal scrap results in credits of the respective raw
to the ceiling with the help of a lifter and some fixation devices.
materials for the primary material portion of the input. The loads
of the waste incineration and recycling processes are assigned
Complementary products for installation include a ceiling beam
to the respective modules (A3, A5 and C3) and not to module
in galvanised steel. This additional product is supplied by
D.
Halton. Their production and packaging are considered in A1,
their transport in A3 and A4 and the end-of-life of their
3.3 Estimates and assumptions
packaging in A5.
Energy and water consumption during production could only be
determined on existing products and not on the average
Others complementary products are used to fix the MUPRO
product.
Ceiling beam (clip, pin, screw). They must be purchased by the
installer because they depend on ceiling type (metallic, 3.4 Cut-off criteria
concrete or wood). They are not considered in this study.
Cut-off criteria follow EN15804 and PCR Part A. No flows have
The application phase considers:
been deliberately omitted from the system boundaries.
- Transportation of material lifter to installation site
- Waste treatment (product packaging) 3.5 Background data
All background data was considered using data from the
Modules B1 & B3-B5 & B7 ecoinvent 3.7.1 (cut-off) database or literary sources.
These modules were considered but evaluated as not relevant
for the products and considered as zero. Products do not 3.6 Data quality
require repair (B3)/replacement (B4)/rehabilitation (B5). Site-specific production data has been collected for 2021 from
the production site. The upstream and downstream processes
The hoods haven't significant impact for emission in indoor air have been modelled based on environmental data from generic
or in water during use. databases ecoinvent. The collected data was reviewed in terms
of consistency, and it is estimated as good quality.
3 Environmental Product Declaration - HALTON FOOD SERVICE - UVI/F MARVEL – Demand Controlled Kitchen Ventilation
other allocations were made in this assessment. The cut-off
3.7 Period under review end-of-life allocation approach was used throughout.
The data is therefore based on 2021. All information is based
on averaged data for 12 consecutive months. 3.10 Comparability
Basically, a comparison or an evaluation of EPD data is only
3.8 Geographic Representativeness possible if all the data sets to be compared were created
Land or region, in which the declared product system is according to EN 15804 and the building context, respectively
manufactured, used or handled at the end of the product´s the product-specific characteristics of performance, are taken
lifespan: Europe into account. According to the EN 15804 standard,
environmental declarations for construction products may not
be comparable if they have not been prepared in accordance
3.9 Allocation
with that standard or if a different notified unit has been
Allocation has been avoided whenever possible by collecting
used.The LCA was conducted using SimaPro 9.2.0.2. software.
product specific environmental data. In case of manufacturing
All background data was considered using data from the
energy use, where allocation could not be avoided, the
ecoinvent 3.7.1 (cut-off) database or literary sources.
consumption of electricity and water in Halton's plant were
allocated per working hours for assembly of each product. No
4. LCA: Scenarios and additional technical information
incineration without energy recovery, 9% landfill.
Characteristic product properties of biogenic carbon
The biogenic carbon content quantifies the amount of biogenic Service Life
carbon in a construction product leaving the factory gate, and it HALTON declares a Service Life of 15 years as an empirical
shall be separately declared for the product and for any value for the hoods when used in accordance with the care
accompanying packaging. instructions.
Maintenance (B2)
The mass of packaging containing biogenic carbon shall is
declared. Name Value Unit
Note: 1 kg of biogenic carbon is equivalent to 44/12 kg of CO . Total number of check-up
2 60
during SRL
Name Value Unit
Estimated distance for round
Biogenic carbon content of the product 0 kg.C 100 km
trip
Biogenic carbon content of associated packaging 15.2 kg.C
Estimated weight of
technician doing the check 80 kg
The scenarios and assumptions applied in this study for all the up.
life cycle stages included are based on data provided by Halton
2 replacements of UV light 5.40E-
and correspond to the most likely scenario. The following kg
during SLR 01
scenarios and general assumptions were made in the studied
3.09E m3 of water containing
lifecycle stages: Weekly cleaning
+03 1,5% soap /DVR
Transport to the building site (A4) Operational energy use (B6)
Name Value Unit Based on a 56h/week usage of the hood.
Transport of distance 1631.4 km Name Value Unit
Capacity utilization (including empty runs) ~19 % Energy demand 1516 kWh/year
Installation into the building (A5) End of life (C1-C4)
Name Value Unit Name Value Unit
Material loss 0 % Transport to treatment site 50 km
The following end of life scenarios are considered for The following end of life scenarios are considered for the
packaging: product:
NHW Wood : 3.00E+01 kg → 31% recycling, 31% incineration
without energy recovery, 38% landfill. NHW Plastic : 1.27E+00 kg → 41% recycling, 37% incineration
without energy recovery, 22% landfill
NHW Plastic : 1.43E+00 kg → 41% recycling, 37% incineration NHW Steel : 1.26E+02 kg → 90% recycling, 10% landfill
without energy recovery, 22% landfill. NHW Glass : 6.97E-01E+02 kg → 100% landfill
NHW WEE : 1.16E+01 kg → 74.7% recycling, 1.8% reuse,
NHW Cardboard : 4.33E+00 kg → 82% recycling, 9% 9.7% incineration without energy recovery, 13.8% landfill
4 Environmental Product Declaration - HALTON FOOD SERVICE - UVI/F MARVEL – Demand Controlled Kitchen Ventilation
5. LCA: Results
The following table shows the result of the LCA for 1 m of a UVI/F MARVEL hood.
DESCRIPTION OF THE SYSTEM BOUNDARY (X = INCLUDED IN LCA; MND = MODULE OR INDICATOR NOT DECLARED; MNR
= MODULE NOT RELEVANT)
Benefits and
Construction loads beyond
Product stage Use stage End of life stage
process stage the system
boundaries
la ire ta m w a Ry lp p u s tro p s n a rT g n iru tc a fu n a M e h t m o rf tro p s n a rTe tis e h t o t e ta g y lb m e s s A e s U e c n a n e tn ia M ria p e R tn e m e c a lp e R tn e m h s ib ru fe R y g re n e la n o ita re p Oe s u re ta w la n o ita re p Oe s u n o itc u rts n o c -e Dn o itilo m e d tro p s n a rT g n is s e c o rp e ts a W la s o p s iD -e s u e R-y re v o c e R-g n ilc y c e Rla itn e to p
A1 A2 A3 A4 A5 B1 B2 B3 B4 B5 B6 B7 C1 C2 C3 C4 D
X X X X X MND X MNR MNR MNR X MND X X X X X
RESULTS OF THE LCA - ENVIRONMENTAL IMPACT according to EN 15804+A2: 1 m UVI/F MARVEL Hood
Parameter Unit A1-A3 A4 A5 B2 B6 C1 C2 C3 C4 D
GWP-total kg CO 2 eq 7.49E+03 3.71E+01 1.14E+02 1.44E+03 9.52E+03 0 1.13E+00 2.51E+00 5.09E+00 -1.94E+02
GWP-fossil kg CO 2 eq 7.51E+03 3.71E+01 4.6E+01 1.27E+03 9.45E+03 0 1.13E+00 3.25E-01 4.36E+00 -1.94E+02
GWP-
biogenic kg CO 2 eq -2.66E+01 1.43E-02 6.8E+01 2.1E+01 5.45E+01 0 4.36E-04 2.18E+00 7.23E-01 -3.43E-01
GWP-luluc kg CO 2 eq 1.2E+01 1.27E-02 2.17E-02 1.45E+02 1.96E+01 0 3.88E-04 4.32E-04 9.06E-05 -7.6E-02
ODP kg CFC11 eq 5.7E-04 8.43E-06 8.64E-06 2.09E-04 4.79E-04 0 2.57E-07 1.21E-07 5.72E-08 -7.6E-06
AP mol H+ eq 4.62E+01 1.03E-01 1.55E-01 7.41E+00 5.16E+01 0 3.15E-03 6.99E-03 2.11E-03 -7.05E-01
EP-
kg P eq 1.26E+00 2.78E-04 4.88E-04 7.82E-01 1E+00 0 8.48E-06 6.48E-05 1.09E-05 -9.62E-03
freshwater
EP-marine kg N eq 9.27E+00 2.1E-02 5.78E-02 3.03E+00 6.88E+00 0 6.41E-04 4.2E-03 1.57E-03 -1.65E-01
EP-terrestrial mol N eq 1.06E+02 2.34E-01 4.75E-01 2.4E+01 7.91E+01 0 7.13E-03 2.68E-02 8.99E-03 -1.79E+00
kg NMVOC
POCP 2.76E+01 8.94E-02 1.51E-01 6.91E+00 2.16E+01 0 2.73E-03 6.22E-03 2.64E-03 -8.85E-01
eq
ADPE kg Sb eq 2.43E+00 1.36E-04 2.61E-04 2.5E-02 8.59E-02 0 4.16E-06 7.31E-05 7.85E-07 -2.71E-04
ADPF MJ 9.57E+04 5.63E+02 6.03E+02 1.79E+04 2E+05 0 1.72E+01 2.9E+00 3.34E+00 -1.9E+03
m3 world eq
WDP 1.8E+03 1.63E+00 2.29E+00 7.67E+02 2.05E+03 0 4.96E-02 -2.33E-01 2.18E-01 1.9E+00
deprived
GWP = Global warming potential; ODP = Depletion potential of the stratospheric ozone layer; AP = Acidification potential of land and water; EP =
Eutrophication potential; POCP = Formation potential of tropospheric ozone photochemical oxidants; ADPE = Abiotic depletion potential for non-fossil
resources; ADPF = Abiotic depletion potential for fossil resources; WDP = Water (user) deprivation potential)
RESULTS OF THE LCA - INDICATORS TO DESCRIBE RESOURCE USE according to EN 15804+A2: 1 m UVI/F MARVEL Hood
Parameter Unit A1-A3 A4 A5 B2 B6 C1 C2 C3 C4 D
PERE MJ 1.17E+04 7.68E+00 1.26E+01 2.13E+03 3.6E+04 0 2.34E-01 1.89E+00 9.21E-02 -2.43E+02
PERM MJ 5.72E+02 0 -2.15E+02 0 0 0 0 0 0 0
PERT MJ 1.22E+04 7.68E+00 -2.03E+02 2.13E+03 3.6E+04 0 2.34E-01 1.89E+00 9.21E-02 -2.43E+02
PENRE MJ 9.56E+04 5.62E+02 6.28E+02 1.81E+04 1.97E+05 0 1.72E+01 2.78E+00 3.34E+00 -1.9E+03
PENRM MJ 1.67E+02 0 -2.52E+01 0 0 0 0 0 -4.79E+00 0
PENRT MJ 9.57E+04 5.62E+02 6.02E+02 1.8E+04 1.97E+05 0 1.72E+01 2.78E+00 -1.45E+00 -1.9E+03
SM kg 7.48E-03 0 0 0 0 0 0 0 0 0
RSF MJ 0 0 0 0 0 0 0 0 0 0
NRSF MJ 0 0 0 0 0 0 0 0 0 0
FW m3 1.16E+02 7.68E-02 1.19E-01 2.64E+01 1.65E+02 0 2.35E-03 -5.92E-04 6.41E-03 -1.34E-01
PERE = Use of renewable primary energy excluding renewable primary energy resources used as raw materials; PERM = Use of renewable primary
energy resources used as raw materials; PERT = Total use of renewable primary energy resources; PENRE = Use of non-renewable primary energy
excluding non-renewable primary energy resources used as raw materials; PENRM = Use of non-renewable primary energy resources used as raw
materials; PENRT = Total use of non-renewable primary energy resources; SM = Use of secondary material; RSF = Use of renewable secondary fuels;
NRSF = Use of non-renewable secondary fuels; FW = Use of net fresh water
RESULTS OF THE LCA – WASTE CATEGORIES AND OUTPUT FLOWS according to EN 15804+A2:
1 m UVI/F MARVEL Hood
Parameter Unit A1-A3 A4 A5 B2 B6 C1 C2 C3 C4 D
HWD kg 1.02E+03 3.87E-01 3.31E+00 7.39E+01 2.21E+02 0 1.18E-02 5.85E-01 2.87E-01 -1.95E+01
NHWD kg 1.06E+04 3.2E+01 3.8E+01 9.98E+02 3.61E+03 0 9.77E-01 2.4E+00 1.29E+01 -4.6E+02
RWD kg 3.08E-01 3.85E-03 4.02E-03 1.03E-01 1.41E+00 0 1.17E-04 9.73E-05 1.82E-05 -3.15E-03
CRU kg 1.29E-01 0 0 7.39E+01 2.21E+02 0 0 5.85E-01 0 -1.95E+01
MFR kg 4.5E+01 0 1.34E+01 9.98E+02 3.61E+03 0 0 2.4E+00 0 -4.6E+02
MER kg 0 0 0 1.03E-01 1.41E+00 0 0 9.73E-05 0 -3.15E-03
EEE MJ 1.02E-04 0 0 0 0 0 0 2.09E-01 0 0
5 Environmental Product Declaration - HALTON FOOD SERVICE - UVI/F MARVEL – Demand Controlled Kitchen Ventilation
EET MJ 0 0 0 0 0 0 0 0 0 0
HWD = Hazardous waste disposed; NHWD = Non-hazardous waste disposed; RWD = Radioactive waste disposed; CRU = Components for re-use;
MFR = Materials for recycling; MER = Materials for energy recovery; EEE = Exported electrical energy; EET = Exported thermal energy
RESULTS OF THE LCA – additional impact categories according to EN 15804+A2-optional:
1 m UVI/F MARVEL Hood
Parameter Unit A1-A3 A4 A5 B2 B6 C1 C2 C3 C4 D
Disease
PM 3.85E-04 2.34E-06 2.11E-06 1.19E-04 1.36E-04 0 7.13E-08 1.06E-07 4.2E-08 -1.22E-05
incidence
IR kBq U235 eq 3.91E+02 2.47E+00 2.66E+00 7.82E+01 1.73E+03 0 7.55E-02 9.12E-02 1.25E-02 -2.86E+00
ETP-fw CTUe 5.99E+05 4.32E+02 5.97E+02 3.55E+04 1.25E+05 0 1.32E+01 3.1E+02 1.06E+02 -4.63E+03
HTP-c CTUh 1.93E-05 1.53E-08 2.54E-08 1.97E-06 3.72E-06 0 4.68E-10 1.6E-09 1.67E-09 -1.18E-06
HTP-nc CTUh 2.39E-04 4.22E-07 5.5E-07 2.23E-05 9.81E-05 0 1.29E-08 4.52E-08 1.9E-08 -4.07E-06
SQP SQP 7.39E+04 5.76E+02 4.24E+02 3.12E+04 6.42E+04 0 1.76E+01 1.16E+02 5.19E+00 -2.47E+03
PM = Potential incidence of disease due to PM emissions; IR = Potential Human exposure efficiency relative to U235; ETP-fw = Potential comparative
Toxic Unit for ecosystems; HTP-c = Potential comparative Toxic Unit for humans (cancerogenic); HTP-nc = Potential comparative Toxic Unit for humans
(not cancerogenic); SQP = Potential soil quality index
Disclaimer 1 – for the indicator “Potential Human exposure efficiency relative to U235”. This impact category deals mainly with the
eventual impact of low-dose ionizing radiation on human health of the nuclear fuel cycle. It does not consider effects due to possible
nuclear accidents, occupational exposure or radioactive waste disposal in underground facilities. Potential ionizing radiation from the
soil, radon and from some construction materials is also not measured by this indicator.
Disclaimer 2 – for the indicators “abiotic depletion potential for non-fossil resources”, “abiotic depletion potential for fossil resources”,
“water (user) deprivation potential, deprivation-weighted water consumption”, “potential comparative toxic unit for ecosystems”,
“potential comparative toxic unit for humans – cancerogenic”, “Potential comparative toxic unit for humans - not cancerogenic”,
“potential soil quality index”. The results of this environmental impact indicator shall be used with care as the uncertainties on these
results are high as there is limited experience with the indicator.
6. LCA: Interpretation
The dominance analysis shows that modules B6 and A1 are the
dominant life cycle stages in most of the categories. B6
dominates most indicators due the energy demand in electricity
for using. The modules A1-A3 have great contributions to all
categories especially for the Depletion of abiotic resources -
minerals and metals. In this indicator the provision of
electronics component has the largest contribution. The end-of-
life stage has no significant influence on the environmental
indicators. The environmental burdens from the transports
(modules A4 and C2) account less than 1% of the total burdens
from the transports in all cases.
7. Requisite evidence
As a general rule, all statements must be documented with If evidence required by the specific PCR part B is not provided,
measured data (presented by the corresponding test this has to be justified under the respective title for the required
certificates). The methods of evidence and the test conditions evidence.
have to be described together with the results.
If relevant for the scope of application of the declared product,
If substances are not detected, the limit of detection must be or if derivable from its material composition, it is recommended
included in the declaration. to provide additional adequate evidence.
Interpreting statements such as “… free of …” or “… are Information and explanation on the representativeness of
entirely harmless …” are not allowed. requisite evidence have to be given in the project report for all
members of the association.
8. References
PCR 2020, Part A on the project report according to EN 15804+A2.
Institut Bauen und Umwelt e.V., Berlin (pub.): Product Version 2020-07.
Category Rule for Construction Products from the www.ibu-epd.com
range of Environmental Product Declarations of
Institute Bauen und Umwelt (IBU), Part A: Calculation PCR 2024, Part B
rules for the Life Cycle Assessment and requirements Product Category Rules for Construction Products,
6 Environmental Product Declaration - HALTON FOOD SERVICE - UVI/F MARVEL – Demand Controlled Kitchen Ventilation
Part B: Ventilations systems for commercial kitchens, Regulation (EC) No. 1907/2006 of the European Parliament
24/01/2024 and of the Council of 18 December 2006 concerning the
Registration, Evaluation, Authorisation and Restriction of
EN 15804 Chemicals (REACH), establishing a European Chemicals
EN 15804:2012+A2:2019+AC:2021, Sustainability of Agency, amending Directive 1999/45/EC and repealing Council
construction works — Environmental Product Declarations — Regulation (EEC) No. 793/93, Commission Regulation (EC) No.
Core rules for the product category of construction products. 1488/94
as well as Council Directive 76/769/EEC and Commission
ISO 14025 Directives 91/155/EEC, 93/67/EEC,
EN ISO 14025:2011, Environmental labels and declarations — 93/105/EC and 2000/21/EC, 2006-12.
Type III environmental declarations — Principles and
procedures. Biocide Guideline
Regulation (EU) No. 528/2012 of the European
DIN 4102-1 Parliament and of the Council of 22 May 2012
DIN 4102-1: Fire behaviour of building materials and building concerning the making available on the market and
components - Part 1: Building materials; concepts, use of biocidal products
requirements and tests. 1998-05
CPR
DIN EN 13501-1 Directive (EU) No. 305/2011 of the European
DIN EN 13501-1:2019-05: Fire classification of construction Parliament and Council dated 9 March 2011
products and building elements - Part 1: Classification using establishing harmonised conditions for marketing
data from reaction to fire tests; German version EN 13501- construction products and replacing Council Guideline
1:2018 89/106/EEC
/Further References Ecoinvent
Ecoinvent database version 3.7.1
SimaPro 9.2.0.2
WEEE IBU 2021
Waste Electrical and Electronic Equipment Directive : Act Institut Bauen und Umwelt e.V.: General Instructions for the
governing the requirements on utilisation and disposal of EPD programme of Institut Bauen und Umwelt e.V., Version
WEEE. 2.0, Berlin: Institut Bauen und Umwelt e.V., 2021
www.ibu-epd.com
REACH Regulation
7 Environmental Product Declaration - HALTON FOOD SERVICE - UVI/F MARVEL – Demand Controlled Kitchen Ventilation
Publisher
Institut Bauen und Umwelt e.V. +49 (0)30 3087748- 0
Hegelplatz 1 info@ibu-epd.com
10117 Berlin www.ibu-epd.com
Germany
Programme holder
Institut Bauen und Umwelt e.V. +49 (0)30 3087748- 0
Hegelplatz 1 info@ibu-epd.com
10117 Berlin www.ibu-epd.com
Germany
Author of the Life Cycle Assessment
CSTB 04 56 14 72 62
rue Joseph Fourier 24 cecile.magnin-feysot@cstb.fr
38400 Saint-Martin-d'Hères https://www.cstb.fr/fr/
France
Owner of the Declaration
HALTON FOODSERVICE 06.14.71.06.55
Zone Technoparc Futura CS 80102 arnaud.kazmierczak@halton.com
62402 BETHUNE Cedex https://www.halton.com/fr/
France
8 Environmental Product Declaration - HALTON FOOD SERVICE - UVI/F MARVEL – Demand Controlled Kitchen Ventilation
