ENVIRONMENTAL PRODUCT DECLARATION
as per ISO 14025 and EN 15804+A2
Owner of the Declaration JANSEN AG
Publisher Institut Bauen und Umwelt e.V. (IBU)
Programme holder Institut Bauen und Umwelt e.V. (IBU)
Declaration number EPD-JAN-20240305-CBA1-EN
Issue date 29.11.2024
Valid to 28.11.2029
Jansen-Economy 60 anti-finger-trap door width x height: 1230 mm
x 2180 mm
Jansen AG
www.ibu-epd.com | https://epd-online.com
General Information
Jansen AG Jansen-Economy 60 anti-finger-trap door width x
height: 1230 mm x 2180 mm
Programme holder Owner of the declaration
IBU – Institut Bauen und Umwelt e.V. JANSEN AG
Hegelplatz 1 Industriestrasse 34
10117 Berlin 9463 Oberriet
Germany Switzerland
Declaration number Declared product / declared unit
EPD-JAN-20240305-CBA1-EN 1 m2 Jansen-Economy 60 anti-finger-trap door with a grammage of 27.21
kg/m². The actual reference size of the declared single leaf door has
dimensions of width x height: 1230 mm x 2180 mm.
This declaration is based on the product category rules: Scope:
Windows and doors , 01.08.2021 The environmental product declaration refers to a single leaf anti-finger-
(PCR checked and approved by the SVR) trap door type Jansen-Economy 60 in specific dimension width x height.
The characteristic values used for the system components Jansen-
Economy 60 in the LCA are provided by Jansen AG.
Issue date
The declared product is defined according to the profile series and product
29.11.2024
characteristics.
The location of the production site is Oberriet/ Switzerland.
Valid to
This EPD was created with the help of a semi-automatic LCA-Tool.
28.11.2029 The owner of the declaration shall be liable for the underlying information
and evidence; the IBU shall not be liable with respect to manufacturer
information, life cycle assessment data and evidences.
The EPD was created according to the specifications of EN 15804+A2. In
the following, the standard will be simplified as EN 15804.
Verification
The standard EN 15804 serves as the core PCR
Independent verification of the declaration and data according to ISO
14025:2011
Dipl.-Ing. Hans Peters internally X externally
(Chairman of Institut Bauen und Umwelt e.V.)
Florian Pronold Matthias Schulz,
(Managing Director Institut Bauen und Umwelt e.V.) (Independent verifier)
1 Environmental Product Declaration - Jansen AG - Jansen-Economy 60 anti-finger-trap door width x height: 1230 mm x 2180 mm
Product
the requirements of an interior or exterior wall without taking
Product description/Product definition over load-bearing functions.
Jansen-Economy 60 anti-finger trap doors have a basic depth
of 60 mm. The rounded half shells minimise the risk of injury at Technical Data
the secondary closing edge. In this way it is possible to prevent According to the CE marking, the following structural data for
crushing and shearing points. Thanks to low-maintenance, the element must be stated:
high-performance hinge bearings, the Jansen Economy 60 anti-
Constructional data
finger-trap doors are particularly suitable for buildings with
Name Value Unit
heavy public use such as shopping centres, schools or
hospitals. The Jansen-Economy 60 anti-finger-trap door meets Operating forces acc. to EN 13115 2 class
the product standard EN 14351-1 for external doors and is CE- Ability to release acc.. to EN 179 / EN requirement
certified. This declaration describes the following element in 1125 fulfilled
Jansen-Economy 60: Smoke control acc. to EN 1634-3 / EN
Sa / S200
Product: Jansen-Economy 60, single leaf anti-finger-trap 13501-2
Face width: 130 mm
Durability of self-closing against ageing
Construction depth: 60 mm achieved
acc. to EN 16034
Width x height: 1230 mm x 2180 mm
Self-closing acc. to EN 16034 / EN
CE marking according to EN 14351-1 C class
13501-2
For the placing on the market in the the European Union/ Product according to the CPR, based on an EN: Performance
European Free Trade Association EU/EFTA the CPR (EU) No. data of the product in accordance with the declaration of
305/2011/ applies. The products require a declaration of performance with respect to its essential characteristics
performance taking into account the harmonized product according to EN 14351-1, doors. Other constructional data are
standard EN 14351-1 windows and doors and a CE marking. not relevant for this product.
The respective national regulations apply to the use. With this
declaration the following element is declared: Base materials/Ancillary materials
JANSEN Jansen-Economy 60 anti-finger-trap door is made of
the following materials:
• Glazing approx. 53%
• Steel approx. 45%
• Plastics and fillers approx. 2%
The percentages relate to the most frequently sold product with
an opening of 2.68 m2. The percentages stated may vary
depending on the product type and dimensions.
Does the product or at least one part product contain materials
from the ECHA candidate list of materials which are especially
problematic for approval: Substances of Very High Concern –
SVHC (date 27.06.2024) above a mass % of 0.1: no.
This product/article/at least one partial article contains other
carcinogenic, mutagenic, reprotoxic (CMR) substances in
categories 1A or 1B which are not on the candidate list,
exceeding 0.1 percentage by mass: no.
Biocide products were added to this construction product or it
has been treated with biocide products (this then concerns a
treated product as defined by the (EU) Ordinance on Biocide
Products No. 528/2012): no.
Reference service life
According to SBR 2011 regarding the specific material
characteristics of steel windows and doors, the reference
service life is 75 years (SBR 2011). The practical service life
may well be longer. Conditions for a long service life are regular
Application maintenance, care and upkeep of the product. The specified
service life is independent of the manufacturer's warranty.
The Jansen-Economy 60 anti-finger-trap door can be integrated
for building ventilation and light transmission and it meets all
LCA: Calculation rules
The declared unit is a 1 m2 of Jansen-Economy 60 anti-finger-
Declared Unit
trap door element.
2 Environmental Product Declaration - Jansen AG - Jansen-Economy 60 anti-finger-trap door width x height: 1230 mm x 2180 mm
The actual reference size of the declared door element has be modified project-specific if required by linear scaling.
dimensions of 1230 mm x 2180 mm.
Modules C3 and C4 - consider waste processing and/or
Declared unit
disposal with the following scenarios:
Name Value Unit
• Scenario 0: 100% thermal treatment of all raw materials
Declared unit 1 m2
with heating value including plastic system parts and
Grammage 27.21 kg/m2 100% recycling of metal system components (C3).
Layer thickness 0.06 m Landfill of all materials without heating value (except
metals) including glazing (C4). For mineral based
Other declared units are allowed if the conversion is shown
components (i.e. gypsum board), construction waste
transparently.
processing (shredding) and material recycling as filling
material (incl. benefits for substitution of gravel in
For inhomogeneous components made of different materials,
Module (D) is considered, assuming 3% recycling
the conversion to other dimensions with factors leads to
losses are sent to landfill (C4).
deviations compared to the exact calculation. The frame
percentage is 30.02% and the ground reference is 0.074m². • Scenario 1 (module C3/1): 100% recycling of plastic
Frame percentage = Frame surface / total area * 100 [%] system parts (excluding e-waste sent to incineration)
Ground reference = Element depth x element width [m²] and 100% recycling of metal system components.
Landfill of all materials without heating value (except
System boundary metals) including glazing (C4/1). For mineral based
Type of EPD according to EN 15804: "cradle to gate with components (i.e. gypsum board), construction waste
options, modules C1–C4, and module D". The following processing (shredding) and material recycling as filling
modules are declared: A1–A3, C, D and additional modules: material (incl. benefits for substitution of gravel in
A4, A5 Module D/1) are considered, assuming 3% recycling
losses are sent to landfill (C4/1).
Production (modules A1-A3):
Modules C4 & C4/1 are identical.
This module considers the provision of all relevant door
components (i.e. metal profiles/components, plastic Benefits and loads beyond the product system boundary
parts/profiles and glazing) and raw materials including their (module D):
transport to the declared production plant. This considers the
manufacturing and assembly of these components, including Considers credits and loads from the recycling of the metal
waste processing up to the end-of-waste state. The impact of components and mineral based components (i.e. gypsum
packaging materials is also covered by this module. board) as filling material (incl. benefits for the substitution of
gravel (duplicated in D and D/1) and the recycling of the plastic
Transport to the construction site (module A4): system parts/profiles (D/1). Avoided burdens from the thermal
treatment of all raw materials with heating value (including
A distance of 100 km is considered for the transport of the plastic system parts/profiles) (D) and packaging treatment
packed finished product via truck. The transport distance can (duplicated in D and D/1) under European conditions are
be modified project-specific if required by linear scaling. considered. This affects only the rate of primary materials (no
secondary materials).
Installation (module A5):
Geographic Representativeness
Treatment and disposal of packaging material is considered in Land or region, in which the declared product system is
this module. Credits for potential avoided burdens due to manufactured, used or handled at the end of the product´s
energy substitution of electricity and thermal energy generation lifespan: Europe
are declared in module D under European conditions and
affects only the rate of primary materials (no secondary
Comparability
materials).
Basically, a comparison or an evaluation of EPD data is only
EoL stage (modules C1-C4): possible if all the data sets to be compared were created
according to EN 15804 and the building context, respectively
Module C1 - considers manual deconstruction (without the product-specific characteristics of performance, are taken
environmental burdens). into account. The following background database has been
used for the LCA calculation: Sphera LCA software (GaBi ts)
Module C2 - considers 50 km truck transport to waste content update package (CUP) version 2022.2
processing. The transport distance can
LCA: Scenarios and additional technical information
Name Value Unit
Characteristic product properties of biogenic carbon
kg
No biogenic carbon is reported in the product. The biogenic Biogenic carbon content in product -
C
carbon content in the accompanying packaging for 1 m2
Biogenic carbon content in accompanying kg
Jansen-Economy 60 anti-finger-trap door is declared below. 0.00703
packaging C
Information on describing the biogenic Carbon Content at
Note: 1 kg of biogenic carbon is equivalent to 44/12 kg of CO .
factory gate 2
The following technical information is a basis for the declared
3 Environmental Product Declaration - Jansen AG - Jansen-Economy 60 anti-finger-trap door width x height: 1230 mm x 2180 mm
modules. The values refer to the declared unit of 1 m2 of losses are sent to landfill (C4).
Jansen-Economy 60 anti-finger-trap door. Scenario 1 considers 100% recycling of plastic system parts
(excluding e-waste sent to incineration) and 100% recycling of
Transport to the building site (A4)
metal system components (C3/1). Landfill of all materials
Name Value Unit without heating value (except metals) including glazing (C4/1).
Litres of fuel 0.051 l/100km For mineral based components (i.e. gypsum board),
Transport distance 100 km construction waste processing (shredding) and material
recycling as filling material (incl. benefits for substitution of
Capacity utilisation (including empty runs) 61 %
gravel in Module D/1) are considered, assuming 3% recycling
Gross weight of packed products transported 27.24 kg
losses are sent to landfill (C4/1). Modules C4 and C4/1 are
identical. The recycling of plastics scenario declared in this
Installation into the building (A5)
EPD is currently considered a scenario that is not widely
Treatment and disposal of packaging material is considered in
available in reality due to economic viability limitations
this module.
associated with higher costs of sorting smaller shares of
The values refer to the declared unit of 1 m2 of Jansen-
plastics such as those present in the declared product.
Economy 60 anti-finger-trap door.
Name Value Unit
Name Value Unit
EoL scenario 0 (modules C3 and C4)
Polyethylene (waste packaging to incineration) 0.00152 kg
Recycling (C3) 12.32 kg
Cardboard box (waste packaging to incineration) 0.00725 kg
Energy recovery (C3) 0.55 kg
Wood (waste packaging to incineration) 0.00957 kg
Landfilling (C4) 14.32 kg
According to SBR 2011 regarding the specific material
EoL scenario 1 (modules C3/1 and C4/1)
characteristics of steel windows and doors, the reference
Recycling (C3/1) 12.87 kg
service life is 75 years (SBR 2011). The practical service life
may well be longer. Conditions for a long service life are regular Energy recovery (C3/1) kg
maintenance, care and upkeep of the product. The specified Landfilling (C4/1) 14.32 kg
service life is independent of the manufacturer's warranty.
Reuse, recovery and/or recycling potentials (D), relevant
Reference service life scenario information
Name Value Unit
Module D includes the credits and loads from the recycling of
Life Span (according to SBR 2011) 75 a
the metal components and mineral based components (i.e.
End of life (C1-C4) gypsum board) as filling material (incl. benefits for substitution
of gravel (duplicated in D and D/1) and the recycling of the
For the End-of-Life stage two scenarios are considered.
plastic system parts/profiles (D/1). Avoided burdens from the
Scenario 0 considers 100% thermal treatment of all raw
thermal treatment of all raw materials with heating value
materials with heating value including plastic system parts and
(including plastic system parts/profiles) (D) and packaging
100% recycling of metal system components (C3). Landfill of all
treatment (duplicated in D and D/1) under European conditions
materials without heating value (except metals) including
are considered. This affects only the rate of primary materials
glazing (C4). For mineral based components (i.e. gypsum
(no secondary materials). A waste incineration plant with R1-
board), construction waste processing (shredding) and material
value > 0.6 is assumed.
recycling as filling material (incl. benefits for substitution of
For recycling, a collection rate of 100% is considered.
gravel in Module D) are considered, assuming 3% recycling
4 Environmental Product Declaration - Jansen AG - Jansen-Economy 60 anti-finger-trap door width x height: 1230 mm x 2180 mm
LCA: Results
Results provided in this section are presented in relation to 1 m2 of anti-finger-trap door type Jansen-Economy 60 (reference
dimensions 1230 mm x 2180 mm).
For the End-of-Life stage, two scenarios are considered:
C3 - considers 100% recycling of metal system components (duplicated in D and D/1) and 100% thermal treatment of all raw materials
with heating value including plastic system parts. For mineral based components (i.e. gypsum board), construction waste processing
(shredding) and material recycling as filling material is considered.
C3/1 - considers 100% recycling of metal system components (duplicated in D and D/1) and 100% recycling of plastic system parts
(excluding e-waste sent to incineration). For mineral based components (i.e. gypsum board), construction waste processing
(shredding) and material recycling as filling material is considered.
C4 and C4/1 - consider landfill of all materials without heating value (except metals) including glazing and recycling losses from mineral
based components (i.e. gypsum board). Modules C4 and C4/1 are identical.
D - considers credits and loads from the recycling of the metal components and mineral based components (i.e. gypsum board) as
filling material (incl. benefits for the substitution of gravel (duplicated in D and D/1). Avoided burdens from packaging treatment
(duplicated in D and D/1) and thermal treatment of all raw materials with heating value (including plastic system parts/profiles) are
considered.
D/1 - considers credits and loads from the recycling of the metal components and mineral based components (i.e. gypsum board) as
filling material (incl. benefits for the substitution of gravel (duplicated in D and D/1) and the recycling of the plastic system parts/profiles.
Avoided burdens from packaging treatment (duplicated in D and D/1) are considered.
DESCRIPTION OF THE SYSTEM BOUNDARY (X = INCLUDED IN LCA; MND = MODULE OR INDICATOR NOT DECLARED; MNR
= MODULE NOT RELEVANT)
Benefits and
Construction loads beyond
Product stage Use stage End of life stage
process stage the system
boundaries
la ire ta m w a Ry lp p u s tro p s n a rT g n iru tc a fu n a M e h t m o rf tro p s n a rTe tis e h t o t e ta g y lb m e s s A e s U e c n a n e tn ia M ria p e R tn e m e c a lp e R tn e m h s ib ru fe R y g re n e la n o ita re p Oe s u re ta w la n o ita re p Oe s u n o itc u rts n o c -e Dn o itilo m e d tro p s n a rT g n is s e c o rp e ts a W la s o p s iD -e s u e R-y re v o c e R-g n ilc y c e Rla itn e to p
A1 A2 A3 A4 A5 B1 B2 B3 B4 B5 B6 B7 C1 C2 C3 C4 D
X X X X X MND MND MNR MNR MNR X MND X X X X X
RESULTS OF THE LCA - ENVIRONMENTAL IMPACT according to EN 15804+A2: 1 m2 Jansen-Economy 60 anti-finger-trap
door (27.21 kg/m2)
Parameter Unit A1-A3 A4 A5 B6 C1 C2 C3 C3/1 C4 C4/1 D D/1
GWP-total kg CO 2 eq 4.43E+01 1.64E-01 3.08E-02 0 0 8.21E-02 1.43E+00 0 2.15E-01 2.15E-01 -1.08E+01 -1.09E+01
GWP-fossil kg CO 2 eq 4.42E+01 1.63E-01 5.24E-03 0 0 8.13E-02 1.43E+00 0 2.14E-01 2.14E-01 -1.08E+01 -1.09E+01
GWP-
biogenic kg CO 2 eq 8.91E-02 6.87E-04 2.55E-02 0 0 3.43E-04 5.41E-05 0 7.2E-04 7.2E-04 2.57E-03 1.65E-03
GWP-luluc kg CO 2 eq 1.45E-02 9.08E-04 8.35E-08 0 0 4.54E-04 5.35E-06 0 3.95E-04 3.95E-04 -2.42E-04 -2.31E-04
kg CFC11
ODP 6.62E-11 9.76E-15 2.64E-15 0 0 4.88E-15 8.39E-14 0 5.02E-13 5.02E-13 -3.35E-12 -9.56E-13
eq
AP mol H+ eq 1.71E-01 1.55E-04 5.76E-06 0 0 7.75E-05 1.38E-04 0 1.52E-03 1.52E-03 -2.26E-02 -2.32E-02
EP-
kg P eq 3.36E-05 4.86E-07 7.14E-10 0 0 2.43E-07 3.65E-08 0 3.62E-07 3.62E-07 -2.54E-06 -1.6E-06
freshwater
EP-marine kg N eq 5.43E-02 4.83E-05 1.93E-06 0 0 2.42E-05 3.58E-05 0 3.88E-04 3.88E-04 -4.06E-03 -4.22E-03
EP-terrestrial mol N eq 6.36E-01 5.8E-04 2.67E-05 0 0 2.9E-04 6.48E-04 0 4.26E-03 4.26E-03 -3.59E-02 -3.77E-02
kg NMVOC
POCP 1.5E-01 1.35E-04 5.2E-06 0 0 6.76E-05 1.02E-04 0 1.18E-03 1.18E-03 -1.63E-02 -1.71E-02
eq
ADPE kg Sb eq 7.98E-05 1.36E-08 6.47E-11 0 0 6.81E-09 2.09E-09 0 2.19E-08 2.19E-08 -2.48E-05 -2.49E-05
ADPF MJ 4.91E+02 2.18E+00 7.26E-03 0 0 1.09E+00 2.23E-01 0 2.8E+00 2.8E+00 -1.03E+02 -1.2E+02
m3 world eq
WDP 3.03E+00 1.46E-03 3.51E-03 0 0 7.31E-04 1.22E-01 0 2.34E-02 2.34E-02 -1.96E+00 -2.02E+00
deprived
GWP = Global warming potential; ODP = Depletion potential of the stratospheric ozone layer; AP = Acidification potential of land and water; EP =
Eutrophication potential; POCP = Formation potential of tropospheric ozone photochemical oxidants; ADPE = Abiotic depletion potential for non-fossil
resources; ADPF = Abiotic depletion potential for fossil resources; WDP = Water (user) deprivation potential)
RESULTS OF THE LCA - INDICATORS TO DESCRIBE RESOURCE USE according to EN 15804+A2: 1 m2 Jansen-Economy 60
anti-finger-trap door (27.21 kg/m2)
Parameter Unit A1-A3 A4 A5 B6 C1 C2 C3 C3/1 C4 C4/1 D D/1
PERE MJ 4.78E+01 1.24E-01 2.55E-01 0 0 6.19E-02 5.29E-02 0 4.2E-01 4.2E-01 3.72E+00 5.33E+00
PERM MJ 2.53E-01 0 -2.53E-01 0 0 0 0 0 0 0 0 0
PERT MJ 4.8E+01 1.24E-01 1.67E-03 0 0 6.19E-02 5.29E-02 0 4.2E-01 4.2E-01 3.72E+00 5.33E+00
PENRE MJ 4.68E+02 2.18E+00 7.7E-02 0 0 1.09E+00 2.37E+01 2.35E+01 2.8E+00 2.8E+00 -1.03E+02 -1.2E+02
PENRM MJ 2.36E+01 0 -6.97E-02 0 0 0 -2.35E+01 -2.35E+01 0 0 0 0
5 Environmental Product Declaration - Jansen AG - Jansen-Economy 60 anti-finger-trap door width x height: 1230 mm x 2180 mm
PENRT MJ 4.92E+02 2.18E+00 7.27E-03 0 0 1.09E+00 2.23E-01 0 2.8E+00 2.8E+00 -1.03E+02 -1.2E+02
SM kg 6.72E+00 0 0 0 0 0 0 0 0 0 5.97E+00 6.25E+00
RSF MJ 0 0 0 0 0 0 0 0 0 0 0 0
NRSF MJ 0 0 0 0 0 0 0 0 0 0 0 0
FW m3 1.04E-01 1.4E-04 8.24E-05 0 0 7E-05 2.87E-03 0 7.12E-04 7.12E-04 -4.52E-02 -4.61E-02
PERE = Use of renewable primary energy excluding renewable primary energy resources used as raw materials; PERM = Use of renewable primary
energy resources used as raw materials; PERT = Total use of renewable primary energy resources; PENRE = Use of non-renewable primary energy
excluding non-renewable primary energy resources used as raw materials; PENRM = Use of non-renewable primary energy resources used as raw
materials; PENRT = Total use of non-renewable primary energy resources; SM = Use of secondary material; RSF = Use of renewable secondary fuels;
NRSF = Use of non-renewable secondary fuels; FW = Use of net fresh water
RESULTS OF THE LCA – WASTE CATEGORIES AND OUTPUT FLOWS according to EN 15804+A2:
1 m2 Jansen-Economy 60 anti-finger-trap door (27.21 kg/m2)
Parameter Unit A1-A3 A4 A5 B6 C1 C2 C3 C3/1 C4 C4/1 D D/1
HWD kg 4.27E-08 1.05E-11 7.1E-13 0 0 5.23E-12 2E-11 0 1.44E-10 1.44E-10 -1.87E-09 -2.63E-09
NHWD kg 1.65E+00 3.13E-04 4.65E-04 0 0 1.56E-04 4.28E-02 0 1.43E+01 1.43E+01 1.44E+00 1.45E+00
RWD kg 1.19E-02 2.69E-06 4.15E-07 0 0 1.34E-06 1.27E-05 0 3.12E-05 3.12E-05 -6.55E-04 -1.78E-04
CRU kg 0 0 0 0 0 0 0 0 0 0 0 0
MFR kg 3.69E-01 0 0 0 0 0 1.23E+01 1.29E+01 0 0 0 0
MER kg 0 0 0 0 0 0 0 0 0 0 0 0
EEE MJ 0 0 3.52E-02 0 0 0 2.21E+00 0 0 0 0 0
EET MJ 0 0 6.3E-02 0 0 0 3.96E+00 0 0 0 0 0
HWD = Hazardous waste disposed; NHWD = Non-hazardous waste disposed; RWD = Radioactive waste disposed; CRU = Components for re-use;
MFR = Materials for recycling; MER = Materials for energy recovery; EEE = Exported electrical energy; EET = Exported thermal energy
RESULTS OF THE LCA – additional impact categories according to EN 15804+A2-optional:
1 m2 Jansen-Economy 60 anti-finger-trap door (27.21 kg/m2)
Parameter Unit A1-A3 A4 A5 B6 C1 C2 C3 C3/1 C4 C4/1 D D/1
Disease
PM 1.41E-06 9.38E-10 3.03E-11 0 0 4.69E-10 1.31E-09 0 1.87E-08 1.87E-08 -3.16E-07 -3.18E-07
incidence
kBq U235
IR 1.93E+00 3.94E-04 6.75E-05 0 0 1.97E-04 2.04E-03 0 3.47E-03 3.47E-03 1.2E-01 2.01E-01
eq
ETP-fw CTUe 9.31E+02 1.51E+00 3.34E-03 0 0 7.56E-01 1.22E-01 0 1.57E+00 1.57E+00 -7.44E+00 -1.71E+01
HTP-c CTUh 8.3E-08 3.05E-11 2.19E-13 0 0 1.52E-11 8.59E-12 0 2.39E-10 2.39E-10 -4.24E-09 -4.43E-09
HTP-nc CTUh 5.54E-07 1.58E-09 8.24E-12 0 0 7.88E-10 3.4E-10 0 2.65E-08 2.65E-08 -1.43E-07 -1.51E-07
SQP SQP 4.3E+01 7.49E-01 2.11E-03 0 0 3.75E-01 6.73E-02 0 5.83E-01 5.83E-01 -3.22E-01 7.15E-01
PM = Potential incidence of disease due to PM emissions; IR = Potential Human exposure efficiency relative to U235; ETP-fw = Potential comparative
Toxic Unit for ecosystems; HTP-c = Potential comparative Toxic Unit for humans (cancerogenic); HTP-nc = Potential comparative Toxic Unit for humans
(not cancerogenic); SQP = Potential soil quality index
Disclaimer 1 – for the indicator 'Potential Human exposure efficiency relative to U235'.This impact category deals mainly with the
eventual impact of low dose ionizing radiation on human health of the nuclear fuel cycle. It does not consider effects due to possible
nuclear accidents, occupational exposure or radioactive waste disposal in underground facilities. Potential ionizing radiation from the
soil, from radon and from some construction materials is also not measured by this indicator.
Disclaimer 2 – for the indicators 'abiotic depletion potential for non-fossil resources', 'abiotic depletion potential for fossil resources',
'water (user) deprivation potential, deprivation-weighted water consumption', 'potential comparative toxic unit for ecosystems', 'potential
comparative toxic unit for humans – cancerogenic', 'Potential comparative toxic unit for humans - not cancerogenic', 'potential soil
quality index'. The results of this environmental impact indicator shall be used with care as the uncertainties on these results are high
as there is limited experience with the indicator. This EPD was created using a software tool.
References
Standards Type III environmental declarations — Principles and
procedures.
EN 14351-1
EN 14351-1:2016, Windows and doors - Product standard, EN 12210
performance characteristics - Part 1: windows and external EN 12210: 2016 Windows and doors - Resistance to wind
pedestrian doorsets loads - classification
EN 16034 EN 12208
EN 16034:2014, pedestrian doorsets, industrial, commercial, DIN EN 12208 Windows and doors - Watertightness -
garage doors and openable windows - Product standard, Classification
performance characteristics - Fire resistance and/or smoke
control characteristics EN ISO 10140
EN ISO 10140-1: 2021 Acoustics - Laboratory measurement of
EN 15804 sound insulation of building elements - Part 1: Application
EN 15804:2012+A2:2019+AC:2021, Sustainability of rulesfor specific products
construction works — Environmental Product Declarations —
Core rules for the product category of construction products. DIN EN ISO 10077-2
DIN EN ISO 10077-2: 2017 Thermal performance of windows,
ISO 14025 doors and shutters - Calculation of thermal transmittance -
EN ISO 14025:2011, Environmental labels and declarations — Part2: Numerical method for frames
6 Environmental Product Declaration - Jansen AG - Jansen-Economy 60 anti-finger-trap door width x height: 1230 mm x 2180 mm
528/2012REGULATION (EU) No 528/2012 OF THE
EN 12207 EUROPEANPARLIAMENT AND OF THE COUNCIL, of 22 May
EN 12207: 2016 Windows and doors - Air permeability - 2012, concerning the making available on the market and use
Classification of biocidal products
EN 1192 SBR 2011
EN 1192: 2000 Doors - Classification of strength requirements SBR life cycle guide [SBR 2011]
EN 1191 Further References
EN 1191: 2012 Windows and doors - Resistance to repeated
opening and closing - Test method Sphera LCA FE Software (GaBi ts)
GaBi ts dataset documentation for the software-system and
EN 1603 databases, LBP, University of Stuttgart and thinkstep,
DIN EN 1603:2013-05 Thermal insulating products for building Leinfelden-Echterdingen, 2023 (https://www.gabi-
applications - Determination of dimensional stability under software.com/support/gabi)
constant normal laboratory conditions
Sphera LCA Calculator Software (GaBi Envision)
EN 13115 GaBi Envision 5.0 Sphera Solution GmbH, the LCA, EPD and
EN 13115: 2020 Windows - Classification of mechanical Ecodesign tool, http://www.gabi-
properties - Racking, torsion and operating forces. software.com/international/software/gabi-envision/, 2022
DIN EN 1634-1
DIN EN 1634-1 Fire resistance and smoke control tests for door
and shutter assemblies, openable windows and elements of Jansen LCA tool
building hardware - Part 1: Fire resistance test for door and LCA tool for façades, windows & door
shutter assemblies and openable windows LCA-Tool No.: IBU-JAN-202301-LT1-EN
Developed by Sphera Solutions GmbH
EN 13501-2 IBU 2021
EN 13501-2: 2021 Fire classification of construction products Institut Bauen und Umwelt e.V.: General Instructions for the
and building elements - Part 2: Classification using data from EPD programme of Institut Bauen und Umwelt e.V., Version
fire resistance and/or smoke control tests, excluding ventilation 2.0, Berlin: Institut Bauen und Umwelt e.V., 2021
services
www.ibu-epd.com
EN 1627
DIN EN 1627:2011-09 Pedestrian doorsets, windows, curtain PCR Part A
walling, grilles and shutters - Burglar resistance - Requirements PCR - Part A: Calculation rules for the Life Cycle Assessment
and classification and Requirements on the Background Report, version 1.3,
Institut Bauen und Umwelt e.V., 08-2021.
ECHA candidate list
ECHA candidate list [BSJ1] - Substances of Very High
Concern– SVHC (date 27.06.2024) PCR Part B
Candidate List of substances of very high concern for PCR – Part B: Requirements on the EPD for Windows and
Authorisation (published in accordance with Article 59(10) ofthe doors, version 1.6, Institut Bauen und Umwelt e.V., 2022
REACH Regulation)REGULATION (EU) No
7 Environmental Product Declaration - Jansen AG - Jansen-Economy 60 anti-finger-trap door width x height: 1230 mm x 2180 mm
Publisher
Institut Bauen und Umwelt e.V. +49 (0)30 3087748- 0
Hegelplatz 1 info@ibu-epd.com
10117 Berlin www.ibu-epd.com
Germany
Programme holder
Institut Bauen und Umwelt e.V. +49 (0)30 3087748- 0
Hegelplatz 1 info@ibu-epd.com
10117 Berlin www.ibu-epd.com
Germany
Author of the Life Cycle Assessment
Sphera Solutions GmbH +49 (0)711 341817-0
Hauptstraße 111- 113 info@sphera.com
70771 Leinfelden-Echterdingen www.sphera.com
Germany
Owner of the Declaration
JANSEN AG 0041717639113
Industriestrasse 34 sustainability@jansen.com
9463 Oberriet www.jansen.com
Switzerland
8 Environmental Product Declaration - Jansen AG - Jansen-Economy 60 anti-finger-trap door width x height: 1230 mm x 2180 mm
