ENVIRONMENTAL PRODUCT DECLARATION
as per ISO 14025 and EN 15804+A2
Owner of the Declaration dormakaba International Holding GmbH
Publisher Institut Bauen und Umwelt e.V. (IBU)
Programme holder Institut Bauen und Umwelt e.V. (IBU)
Declaration number EPD-DOR-20230256-CBA2-EN
Issue date 25.07.2023
Valid to 24.07.2028
PURE Sonos
dormakaba
www.ibu-epd.com | https://epd-online.com
General Information
dormakaba PURE Sonos
Programme holder Owner of the declaration
IBU – Institut Bauen und Umwelt e.V. dormakaba International Holding GmbH
Hegelplatz 1 DORMA Platz 1
10117 Berlin 58256 Ennepetal
Germany Germany
Declaration number Declared product / declared unit
EPD-DOR-20230256-CBA2-EN 1 piece of the product: Framed Glass Wall System PURE Sonos,
consisting of the following items:
• Framed Glass Wall System
• Product Packaging
This declaration is based on the product category rules: Scope:
Building Hardware products, 01.08.2021 This EPD refers to a specific framed glass wall system manufactured by
(PCR checked and approved by the SVR) dormakaba. The production site is located in Reamstown (USA).
The data represents the dormakaba financial year 2022.
Issue date
The owner of the declaration shall be liable for the underlying information
25.07.2023
and evidence; the IBU shall not be liable with respect to manufacturer
information, life cycle assessment data and evidences.
Valid to
The EPD was created according to the specifications of EN 15804+A2. In
24.07.2028 the following, the standard will be simplified as EN 15804.
Verification
The standard EN 15804 serves as the core PCR
Independent verification of the declaration and data according to ISO
14025:2011
internally X externally
Dipl.-Ing. Hans Peters
(Chairman of Institut Bauen und Umwelt e.V.)
Florian Pronold Matthias Klingler,
(Managing Director Institut Bauen und Umwelt e.V.) (Independent verifier)
1 Environmental Product Declaration - dormakaba - PURE Sonos
Product
The product with respect to its characteristics are in accordance
Product description/Product definition with the relevant technical provisions (no CE-marking):
PURE Sonos Framed Glass Wall Systems provide the
• Americans with Disabilities Act (ADA)
transparency of glass combined with STC rating to enhance
privacy. With an innovative blend of metal and glass, the PURE Base materials/Ancillary materials
Sonos design fully frames the glass panels, adding rigidity and
The major material composition including the packaging of the
greater sound protection without interrupting sight lines.
product is listed below:
Name Value Unit
For the use and application of the product, the respective
national provisions at the place of use Aluminium 80 %
apply: Paper 8 %
• Sound Transmission Class (STC) Steel 7 %
• Americans with Disabilities Act (ADA) Plastics 4 %
Others <1 %
Application
PURE Sonos Framed Glass Walls are ideal for:
The product/s include/s partial articles which contain
• Spaces requiring greater sound control
substances listed in the Candidate List of REACH Regulation
• Sliding door applications
1907/2006/EC (date: 17.01.2023) exceeding 0.1 percentage by
• Office fronts
mass: No.
• Small conference rooms
Reference service life
Technical Data
The reference service life for PURE Sonos amounts to 10 years
PURE Sonos Framed Glass Walls have the following technical
and depends on the application and frequency of use. For
properties:
repairs or renewals, suitable spare parts are available. PURE
Sonos is tested and designed to withstand a minimum of
1.500.000 cycles.
LCA: Calculation rules
Construction stage - Modules A4-A5
Declared Unit The construction process stage includes:
The declared unit is 1 piece of the product including packaging: — A4, transport to the building site;
PURE Sonos. — A5, treatment of waste packaging materials arising
during installation into the building.
Name Value Unit
Declared unit 1 piece/product
End-of-life stage– Modules C1-C4 and D
Weight of declared unit 33,66 kg
The end-of-life stage includes:
— C1, de-construction, demolition;
— C2, transport to waste processing;
System boundary
— C3, waste processing for reuse, recovery and/or
The type of EPD is according to EN 15804: "cradle to
recycling;
gate with options, modules C1–C4, and module D".
— C4, disposal;
The following modules are declared: A1-A3, C, D and
including provision and all transport, provision of all
additional modules: A4 + A5
materials, products and related energy and water use.
Module D (Benefits and loads beyond the system
Production - Module A1-A3
boundary) includes:
The product stage includes:
— D, recycling potentials, expressed as net impacts
— A1, raw material extraction, processing of
and benefits.
secondary material input (e.g. recycling processes),
— A2, transport to the manufacturer, Geographic Representativeness
— A3, manufacturing and assembly, processing and Land or region, in which the declared product system is
mechanical treatments, manufactured, used or handled at the end of the product´s
including provision of all materials, products and lifespan: United States
energy, as well as waste processing up to the end-of waste
state.
Comparability
2 Environmental Product Declaration - dormakaba - PURE Sonos
Basically, a comparison or an evaluation of EPD data is only the product-specific characteristics of performance, are taken
possible if all the data sets to be compared were created into account. Background database: GaBi, SP40
according to EN 15804 and the building context, respectively
LCA: Scenarios and additional technical information
Reference service life
Characteristic product properties of biogenic carbon
Name Value Unit
Name ValueUnit
Life Span according to the manufacturer 10 a
kg
Biogenic carbon content in product 0.06
C
End of life (C1-C4)
Biogenic carbon content in accompanying kg
0.99 C1: The product dismantling from the building is done manually
packaging C
without environmental burden.
C2: Transport to waste treatment at end of life is 50 km.
Name Value Unit
Collected separately waste type 31 kg
Transport to the building site (A4) Recycling 29.7 kg
Name Value Unit Energy recovery 1.3 kg
Litres of fuel 0.00276 l/100km
The product is disassembled in a recycling process. Material
Transport distance 100 km recycling is then assumed for the metals. The plastic
Capacity utilisation (including empty runs) 55 % components are assumed to be incinerated with energy
recovery. Minor proportions of residues arising from the
The product is transported via truck. The main distribution
recycling process are landfilled (1 %). Region for the End of Life
region is US. In order to allow scaling to a specific point of
is: Global.
installation 100 km are declared.
Reuse, recovery and/or recycling potentials (D), relevant
Installation into the building (A5)
scenario information
Name Value Unit
Name Value Unit
Waste packaging (Paper) 2.7 kg
Recycling 100 %
The collection rate is 100 %.
3 Environmental Product Declaration - dormakaba - PURE Sonos
LCA: Results
DESCRIPTION OF THE SYSTEM BOUNDARY (X = INCLUDED IN LCA; ND = MODULE OR INDICATOR NOT DECLARED; MNR =
MODULE NOT RELEVANT)
Benefits and
Construction loads beyond
Product stage Use stage End-of-life stage
process stage the system
boundaries
la ire ta m w a Ry lp p u s tro p s n a rT g n iru tc a fu n a M e h t m o rf tro p s n a rTe tis e h t o t e ta g y lb m e s s A e s U e c n a n e tn ia M ria p e R tn e m e c a lp e R tn e m h s ib ru fe R y g re n e la n o ita re p Oe s u re ta w la n o ita re p Oe s u n o itc u rts n o c -e Dn o itilo m e d tro p s n a rT g n is s e c o rp e ts a W la s o p s iD -e s u e R-y re v o c e R-g n ilc y c e Rla itn e to p
A1 A2 A3 A4 A5 B1 B2 B3 B4 B5 B6 B7 C1 C2 C3 C4 D
X X X X X MND MND MNR MNR MNR MND MND X X X X X
RESULTS OF THE LCA - ENVIRONMENTAL IMPACT according to EN 15804+A2: 1 piece PURE Sonos
Parameter Unit A1-A3 A4 A5 C1 C2 C3 C4 D
GWP-total kg CO 2 eq 2.58E+02 2.94E-01 3.83E+00 0 1.35E-01 3.48E+00 0 -1.62E+02
GWP-fossil kg CO 2 eq 2.62E+02 2.81E-01 9.59E-02 0 1.29E-01 3.21E+00 0 -1.62E+02
GWP-biogenic kg CO 2 eq -4.45E+00 1.3E-02 3.73E+00 0 5.98E-03 2.69E-01 0 -5.27E-01
GWP-luluc kg CO 2 eq 1.16E-01 6.7E-06 6.3E-05 0 3.08E-06 1.84E-04 0 -2.52E-02
ODP kg CFC11 eq 1.01E-10 2.97E-17 6.9E-16 0 1.37E-17 1.65E-15 0 -1.33E-09
AP mol H+ eq 1.24E+00 2.82E-04 1.07E-03 0 1.3E-04 6.09E-04 0 -6.18E-01
EP-freshwater kg P eq 2.19E-04 6.02E-08 1.35E-07 0 2.77E-08 2.63E-07 0 -8.09E-05
EP-marine kg N eq 1.78E-01 8.96E-05 3.87E-04 0 4.12E-05 1.41E-04 0 -8.03E-02
EP-terrestrial mol N eq 1.94E+00 9.96E-04 4.83E-03 0 4.58E-04 2.78E-03 0 -8.73E-01
kg NMVOC
POCP 5.48E-01 2.53E-04 1.03E-03 0 1.17E-04 3.9E-04 0 -2.53E-01
eq
ADPE kg Sb eq 2.33E-04 8.44E-09 1.09E-08 0 3.88E-09 2.27E-08 0 -4.77E-05
ADPF MJ 3.44E+03 3.99E+00 1.21E+00 0 1.84E+00 1.54E+00 0 -2.34E+03
m3 world eq
WDP 3.77E+01 5.51E-04 4.75E-01 0 2.54E-04 3.56E-01 0 -7.08E+00
deprived
GWP = Global warming potential; ODP = Depletion potential of the stratospheric ozone layer; AP = Acidification potential of land and water; EP =
Eutrophication potential; POCP = Formation potential of tropospheric ozone photochemical oxidants; ADPE = Abiotic depletion potential for non-fossil
resources; ADPF = Abiotic depletion potential for fossil resources; WDP = Water (user) deprivation potential)
RESULTS OF THE LCA - INDICATORS TO DESCRIBE RESOURCE USE according to EN 15804+A2: 1 piece PURE Sonos
Parameter Unit A1-A3 A4 A5 C1 C2 C3 C4 D
PERE MJ 1.45E+03 1.26E-02 3.26E+01 0 5.79E-03 2.2E+00 0 -1.13E+03
PERM MJ 3.42E+01 0 -3.24E+01 0 0 -1.8E+00 0 0
PERT MJ 1.48E+03 1.26E-02 2.2E-01 0 5.79E-03 3.97E-01 0 -1.13E+03
PENRE MJ 3.4E+03 3.99E+00 1.21E+00 0 1.84E+00 4.15E+01 0 -2.34E+03
PENRM MJ 4E+01 0 0 0 0 -4E+01 0 0
PENRT MJ 3.44E+03 3.99E+00 1.21E+00 0 1.84E+00 1.54E+00 0 -2.34E+03
SM kg 2.72E+00 0 0 0 0 0 0 0
RSF MJ 0 0 0 0 0 0 0 0
NRSF MJ 0 0 0 0 0 0 0 0
FW m3 3.43E+00 2.26E-05 1.12E-02 0 1.04E-05 8.5E-03 0 -1.96E+00
PERE = Use of renewable primary energy excluding renewable primary energy resources used as raw materials; PERM = Use of renewable primary
energy resources used as raw materials; PERT = Total use of renewable primary energy resources; PENRE = Use of non-renewable primary energy
excluding non-renewable primary energy resources used as raw materials; PENRM = Use of non-renewable primary energy resources used as raw
materials; PENRT = Total use of non-renewable primary energy resources; SM = Use of secondary material; RSF = Use of renewable secondary fuels;
NRSF = Use of non-renewable secondary fuels; FW = Use of net fresh water
RESULTS OF THE LCA – WASTE CATEGORIES AND OUTPUT FLOWS according to EN 15804+A2:
1 piece PURE Sonos
Parameter Unit A1-A3 A4 A5 C1 C2 C3 C4 D
HWD kg 3.72E-06 3.87E-10 1.78E-09 0 1.78E-10 5.7E-09 0 -1.07E-06
NHWD kg 6.8E+01 4.08E-04 1.2E-01 0 1.88E-04 3.35E-01 0 -4.44E+01
RWD kg 2.03E-01 4.29E-06 6.35E-05 0 1.97E-06 5.85E-05 0 -2.69E-01
CRU kg 0 0 0 0 0 0 0 0
MFR kg 0 0 0 0 0 2.96E+01 0 0
MER kg 0 0 0 0 0 0 0 0
EEE MJ 0 0 5.79E+00 0 0 6.32E+00 0 0
EET MJ 0 0 1.05E+01 0 0 1.43E+01 0 0
4 Environmental Product Declaration - dormakaba - PURE Sonos
HWD = Hazardous waste disposed; NHWD = Non-hazardous waste disposed; RWD = Radioactive waste disposed; CRU = Components for re-use;
MFR = Materials for recycling; MER = Materials for energy recovery; EEE = Exported electrical energy; EET = Exported thermal energy
RESULTS OF THE LCA – additional impact categories according to EN 15804+A2-optional:
1 piece PURE Sonos
Parameter Unit A1-A3 A4 A5 C1 C2 C3 C4 D
Disease
PM 1.27E-05 1.48E-09 5.94E-09 0 6.81E-10 7.47E-09 0 -1E-05
incidence
IR kBq U235 eq 4.05E+01 6.13E-04 9.83E-03 0 2.82E-04 5.49E-03 0 -5.44E+01
ETP-fw CTUe 1.25E+03 2.83E+00 5.74E-01 0 1.3E+00 5.83E-01 0 -8.9E+02
HTP-c CTUh 1.72E-07 5.32E-11 3.03E-11 0 2.45E-11 4.99E-11 0 -4.36E-08
HTP-nc CTUh 3.85E-06 2.28E-09 1.31E-09 0 1.05E-09 4.94E-09 0 -1.17E-06
SQP SQP 8.18E+02 1.03E-02 3.2E-01 0 4.72E-03 4.61E-01 0 -6.89E+01
PM = Potential incidence of disease due to PM emissions; IR = Potential Human exposure efficiency relative to U235; ETP-fw = Potential comparative
Toxic Unit for ecosystems; HTP-c = Potential comparative Toxic Unit for humans (cancerogenic); HTP-nc = Potential comparative Toxic Unit for humans
(not cancerogenic); SQP = Potential soil quality index
Disclaimer 1 – for the indicator “Potential Human exposure efficiency relative to U235”. This impact category deals mainly with the
eventual impact of low-dose ionizing radiation on human health of the nuclear fuel cycle. It does not consider effects due to possible
nuclear accidents, occupational exposure or radioactive waste disposal in underground facilities. Potential ionizing radiation from the
soil, radon and from some construction materials is also not measured by this indicator.
Disclaimer 2 – for the indicators “abiotic depletion potential for non-fossil resources”, “abiotic depletion potential for fossil resources”,
“water (user) deprivation potential, deprivation-weighted water consumption”, “potential comparative toxic unit for ecosystems”,
“potential comparative toxic unit for humans – cancerogenic”, “Potential comparative toxic unit for humans - not cancerogenic”,
“potential soil quality index”. The results of this environmental impact indicator shall be used with care as the uncertainties on these
results are high as there is limited experience with the indicator.
This EPD was created using a software tool.
References
ADA 2.0., Berlin: Institut Bauen und Umwelt e.V., 2021. www.ibu-
Americans with Disabilities Act 1990 https://www.ada.gov/ epd.com
STC LCA-tool dormakaba
Sound Transmission Class LCA tool IBU-DOR-202106-LT1-EN, 2021, developed by
Sphera Solutions GmbH
EN 15804
EN 15804:2019+A2, Sustainability of construction works — GaBi ts software
Environmental Product Declarations — Core rules for the Sphera Solutions GmbH
product category of construction products Gabi Software System and Database for Life Cycle Engineering
1992-2020 Version 10.0.0.71
ISO 14025 University of Stuttgart Leinfelden-Echterdingen
DIN EN ISO 14025:2011-10, Environmental labels and
declarations — Type III environmental declarations — GaBi ts documentation
Principles and procedures GaBi life cycle inventory data documentation
(https://www.gabisoftware.com/support/gabi/gabidatabase-
Registration, Evaluation, Authorisation and Restriction of 2020-lci-documentation/)
Chemicals (REACH)
Regulation (EC) No 1907/2006 of the European Parliament and PCR Part A
of the Council on the Registration, Evaluation, Authorisation PCR – Part A: Calculation Rules for the Life Cycle
and Restriction of Chemicals (REACH) Assessment and Requirements on the Project Report according
to EN 15804+A2:2019
Further References PCR Part B
PCR-
IBU 2021 Part B: Requirements on the EPD for BuildingHardware
Institut Bauen und Umwelt e.V.: General Instructions for the products, version 08/21, Institut Bauen und Umwelt e.V.,
EPDs programme of Institut Bauen und Umwelt e.V. Version www.ibu-epd.com.
5 Environmental Product Declaration - dormakaba - PURE Sonos
Publisher
Institut Bauen und Umwelt e.V. +49 (0)30 3087748- 0
Hegelplatz 1 info@ibu-epd.com
10117 Berlin www.ibu-epd.com
Germany
Programme holder
Institut Bauen und Umwelt e.V. +49 (0)30 3087748- 0
Hegelplatz 1 info@ibu-epd.com
10117 Berlin www.ibu-epd.com
Germany
Author of the Life Cycle Assessment
dormakaba International Holding GmbH +49 2333 793-0
DORMA Platz 1 info.de@dormakaba.com
58256 Ennepetal www.dormakaba.com
Germany
Owner of the Declaration
dormakaba International Holding GmbH +49 2333 793-0
DORMA Platz 1 info.de@dormakaba.com
58256 Ennepetal www.dormakaba.com
Germany
6 Environmental Product Declaration - dormakaba - PURE Sonos
