ENVIRONMENTAL PRODUCT DECLARATION
as per ISO 14025 and EN 15804+A2
Owner of the Declaration Interface Europe Manufacturing BV
Publisher Institut Bauen und Umwelt e.V. (IBU)
Programme holder Institut Bauen und Umwelt e.V. (IBU)
Declaration number EPD-INT-20220234-CBB2-EN
Issue date 27.04.2023
Valid to 16.02.2028
Tufted tiles, 100% recycled Polyamid 6 with a maximum total pile
weight of 1500 g/m2, a CQuest Bio Sone+ backing
Interface
www.ibu-epd.com | https://epd-online.com
General Information
Interface Tufted tiles, 100% recycled Polyamid 6 with a
maximum total pile weight of 1500 g/m2, a CQuest
Bio Sone+ backing
Programme holder Owner of the declaration
IBU – Institut Bauen und Umwelt e.V. Interface Europe Manufacturing BV
Hegelplatz 1 Industrielaan 15
10117 Berlin 3925ZG Scherpenzeel
Germany Netherlands
Declaration number Declared product / declared unit
EPD-INT-20220234-CBB2-EN 1 m² tufted modular carpet tiles with Sone+ acoustic felt covered CQuest
Bio (CQB) heavy backing and a pile material of PA 6 with 100% recycled
content
This declaration is based on the product category rules: Scope:
Floor coverings, 01.08.2021 The manufacturer declaration applies to tufted carpet tiles with a Sone+
(PCR checked and approved by the SVR) polyester felt covered CQuest Bio backing, a pile material of 100%
recycled PA 6 with a maximum total pile weight of 1500 g/m2. The products
are tufted in Scherpenzeel, the Netherlands, or in Craigavon, Ireland. The
Issue date carpets are back coated in Scherpenzeel.
27.04.2023 LCA results for products with a maximum total pile weight of 535 g/m2 can
be taken from the corresponding tables of the annexe. Specific data for
every product within the declared group of products in relation to its total
Valid to pile weight can be calculated by using equation 1 given in the annexe (see
annexe chapter: 'General Information on the annexe'). The declaration is
16.02.2028 only valid in conjunction with a valid GUT-PRODIS license of the product.
The owner of the declaration shall be liable for the underlying information
and evidence; the IBU shall not be liable with respect to manufacturer
information, life cycle assessment data and evidences.
The EPD was created according to the specifications of EN 15804+A2. In
the following, the standard will be simplified as EN 15804.
Verification
The standard EN 15804 serves as the core PCR
Independent verification of the declaration and data according to ISO
Dipl.-Ing. Hans Peters 14025:2011
(Chairman of Institut Bauen und Umwelt e.V.)
internally X externally
Florian Pronold Prof. Dr. Birgit Grahl,
(Managing Director Institut Bauen und Umwelt e.V.) (Independent verifier)
1 Environmental Product Declaration - Interface - Tufted tiles, 100% recycled Polyamid 6 with a maximum total pile weight of 1500 g/m2, a CQuest Bio Sone+ backing
Product
Performance data of the product in accordance with the
Product description/Product definition declaration of performance with respect to its essential
The declaration applies to tufted carpet tiles having a surface characteristics according to EN 14041: 2018-05, Resilient,
pile of 100% recycled solution dyed polyamide 6 with a textile and laminate floor coverings - Essential characteristics.
maximum total pile weight of 1050 g/m2. The backing of the Additional product properties in accordance with EN 1307 can
carpet consists of a CQuest Bio backing covered by a Sone+ be found on the Product Information System PRODIS using the
acoustic felt. The total recycled content of the carpet is 82%. PRODIS registration number of the product (www.pro-dis.info)
CQuest Bio backing system Sone+: or on the manufacturer's technical information section.
Backing compound based on renewable wood resin, containing
a recycled filler, glass-fleece reinforcement and polyester Base materials/Ancillary materials
covering fleece. For the placing on the market of the specific Name Value Unit
product in the European Union/European Free Trade Polyamide 6 28.3 %
Association (EU/EFTA) (with the exception of Switzerland)
Polyester 19.3 %
Regulation (EU) No. 305/2011 Construction Product Regulation
Ethylene vinyl acetate (EVA) 4.5 %
(CPR) applies. The product needs a Declaration of
Performance (DoP) taking into consideration EN 14041:2018- Wood resin 5.3 %
05, Resilient, textile and laminate floor coverings - Essential Additives 1.4 %
characteristics, and the CE-marking. The DoP of the product Limestone 36.9 %
can be found on the manufacturer's technical information
Aluminiumhydroxide 3.9 %
section. For the application and use of the product the
Glass fiber 0.4 %
respective national provisions apply.
The specific product covered by the EPD contains substances
Application listed in the ECHA candidate list (08.07.2021) exceeding 0.1
The use class of the specific product as defined in EN 1307 can percentage by mass: no This product contains other CMR
be found in the Product Information System (PRODIS) using substances in categories 1A or 1B which are not on the
the PRODIS registration number of the product. candidate list exceeding 0.1 percentage by mass: no
Biocide products were added to this construction product or it
Technical Data
has been treated with biocide products (this then concerns a
The performance data listed in the Declaration of Performance treated product as defined by the (EU) Ordinance on Biocide
(DoP) apply. Products No. 528/2012): no
Constructional data according to EN 1307 Aluminium hydroxide is used as fire retardant.
Name Value Unit
Reference service life
Product Form Modular carpet tiles, 50 cm x 50 cm -
The service life of textile floor coverings strongly depends on
Type of the correct installation taking into account the declared use
Tufted carpet -
manufacture classification and the adherence to cleaning and maintenance
Polyamide 6 from 100% recycled instructions.
Yarn type -
material A calculation of the reference service life according to ISO
Total carpet 15686 is not possible. Alternatively, a reference service life of
weight 5294 g/m2 15 years can be assumed, during which the functional and
visual quality is guaranteed (In accordance with the warranty of
Secondary CQuest Bio backing with acoustic
- the manufacturer). The technical service life can be significantly
backing textile bottom Sone+
longer.
LCA: Calculation rules
the PRODIS
Declared Unit registration number of the product (www.pro-dis.info) or on the
The indicated values refer to a virtual reference product with the manufacturer's technical information section.
max. total pile weight and the max. total weight.
Name Value Unit
System boundary
Declared unit 1 m2
Type of EPD: Cradle-to-gate with options System boundaries of
Grammage (declared virtual product) 5.294 kg/m2 modules A, B, C, D:
Layer thickness 0.011 m Modules C3, C4 and D are indicated separately for three end-
Total thickness (heaviest real product) 11 mm of-life scenarios:
1 - landfill disposal
Gross density (heaviest real product) 416 kg/m3
2 - municipal waste incineration
The declared unit refers to 1 m2 produced textile floor covering. 3 - recovery in a cement plant
The output of module A5 'Assembly' is 1 m2 installed textile A1-A3 Production:
floor covering. Energy supply and production of the basic material, processing
As the thickness of a virtual product cannot be calculated due of secondary material, auxiliary material, transport of the
to the fact that the total thickness does not depend on the total material to the manufacturing site, emissions, waste water
weight, the declared total thickness and gross density refer to treatment, packaging material and waste processing up to the
the heaviest real product. landfill disposal of residual waste (except radioactive waste).
The layer thickness of the specific product covered by the EPD Benefits for generated electricity and steam due to the
can be found on the Product Information System PRODIS using incineration of production waste are aggregated. Biogenic
2 Environmental Product Declaration - Interface - Tufted tiles, 100% recycled Polyamid 6 with a maximum total pile weight of 1500 g/m2, a CQuest Bio Sone+ backing
carbon that is stored in renewable material (wood resin,
renewable additives,packaging paper) is taken into account as C2 Transport:
well as the associated carbon dioxide uptake from the air from Transport of the carpet waste to a landfill, to the municipal
which this biogenic carbon comes. waste incineration plant (MWI) or to the waste collection facility
for recycling.
A4 Transport:
Transport of the packed textile floor covering from factory gate C3 Waste processing:
to the place of installation. C3-1: Landfill disposal needs no waste processing.
C3-2: Impact from waste incineration (plant with R1 > 0.6),
A5 Installation: generated electricity and steam are listed in the result table as
Installation of the textile floor covering, processing of exported energy.
installation waste and packaging waste up to the landfill C3-3:
disposal of residual waste (except radioactive waste), the Collection of the carpet waste for recovery in the cement
production of the amount of carpet that occurs as installation industry, waste processing (granulating), transport to the
waste including its transport to the place of installation. cement plant, emissions from the incineration.
Generated electricity and steam due to the incineration of
waste are listed in the result table as exported energy. Biogenic C4 Disposal
carbon that is stored in renewable materials in installation C4-1: Impact from landfill disposal,
waste and packaging paper is released as carbon dioxide C4-2: The carpet waste leaves the system in module C3-2,
emissions into the air at the end of life in module A5. C4-3: The pre-processed carpet waste leaves the system in
Preparation of the floor and auxiliary materials (adhesives, module C3-3.
fixing agents, PET connectors) are beyond the system
boundaries and not taken into account. D Recycling potential:
Calculated benefits result from materials exclusive secondary
B1 Use: materials (net materials).
Indoor emissions during the use stage. After the first year, no D-A5: Benefits for generated energy due to incineration of
product-related Volatile Organic Compound (VOC) emissions packaging and installation waste (incineration plant with R1 >
are relevant due to known VOC decay curves of the product. 0.6),
D-1: Assuming that the chemically bound renewable materials
B2 Maintenance: in a landfill gas do not release landfill gas within 100 years, no
Cleaning of the textile floor covering for a period of 1 year: benefits due to landfill dosposal of carpet waste at the end-of-
Vacuum cleaning – electricity supply life are taken into account,
Wet cleaning – electricity, water consumption, production of the D-2: Benefits for generated energy due to incineration of carpet
cleaning agent, waste water treatment waste at the end-of-life (incineration plant with R1 > 0.6),
The declared values in this module have to be multiplied by the D-3: Benefits for saved fossil energy and saved inorganic
assumed service life of the floor covering in the building in material due to recovery of the carpet in a cement plant.
question.
Geographic Representativeness
B3 - B5: Land or region, in which the declared product system is
The modules are not relevant within the assumed reference manufactured, used or handled at the end of the product´s
service life of 15 years. lifespan: Europe
B6 - B7:
Comparability
No energy and water input are required for the operation of the
Basically, a comparison or an evaluation of EPD data is only
carpet in the use stage. The modules do not cause any
possible if all the data sets to be compared were created
environmental impact.
according to EN 15804 and the building context, respectively
the product-specific characteristics of performance, are taken
C1 De-construction:
into account.
The floor covering is de-constructed manually and no additional
environmental impact is caused.
LCA: Scenarios and additional technical information
Name Value Unit
Characteristic product properties of biogenic carbon
Litres of fuel (truck, EURO 0-6 mix) 0.012 l/100km
Name ValueUnit
Transport distance 700 km
kg
Biogenic carbon content in product at factory gate 0.26 Capacity utilisation (including empty runs) 55 %
C
Biogenic carbon content in accompanying kg Installation in the building (A5)
0.05
packaging at factory gate C
Name Value Unit
1 kg biogenic Carbon is equivalent to 44/12 kg of CO 2 Material loss 0.159 kg
Polyethylene packaging waste and installation waste are
considered to be incinerated in a municipal waste incineration
plant. Cardboard packaging waste is going to be recycled.
Preparation of the floor and auxiliaries (adhesives, fixing
Transport to the construction site (A4)
agents, PET connectors etc.) are not taken into account.
Maintenance (B2)
3 Environmental Product Declaration - Interface - Tufted tiles, 100% recycled Polyamid 6 with a maximum total pile weight of 1500 g/m2, a CQuest Bio Sone+ backing
The values for cleaning refer to 1 m2 floor covering per year. End of Life (C1-C4)
Depending on the application based on ISO 10874, the
Three different end-of-life scenarios are declared and the
technical service life recommended by the manufacturer and
results are indicated separately in module C.
the anticipated strain on the floor by customers, the case-
Each scenario is calculated as a 100% scenario.
specific useful life can be established. Based on this useful life
Scenario 1: 100 % landfill disposal
the effects of module B2 need to be calculated in order to
Scenario 2: 100 % municipal waste incineration (MWI)
obtain the overall environmental impacts.
with R1 > 0.6
Name Value Unit Scenario 3: 100 % recovery in the cement industry
Maintenance cycle (vacuum cleaning) 208 Number /year
Maintenance cycle (wet cleaning) 1,5 Number /year If combinations of these scenarios have to be calculated this
should be done according to the following scheme:
Water consumption (wet cleaning) 0.004 m3
EOL-impact = x % impact (Scenario 1)
Cleaning agent (wet cleaning) 0.09 kg + y % impact (Scenario 2)
Electricity consumption 0.314 kWh + z % impact (Scenario 3)
with x % + y % + z % = 100 %
For further information on cleaning and maintenance see
www.interface.com
Name ValueUnit
. Collected as mixed construction waste (scenario 1
5.294 kg
Service life and 2)
Collected separately (scenario 3) 5.294 kg
Name Value Unit
Landfilling (scenario 1) 5.294 kg
Life Span (according to
15 a
manufacturer's warranty) Energy recovery (scenario 2) 5.294 kg
Corresponds to the Energy recovery (scenario 3) 2,464 kg
Declared product properties (at
specifications of EN - Recycling (scenario 3) 2.18 kg
the gate) and finishes
1307
Reuse, recovery and/or recycling potentials (D), relevant
An assumed quality of work,
Conforms to the scenario information
when installed in accordance
manufacturer's - Recovery or recycling potentials due to the three end-of-life
with the manufacturer’s
instructions scenarios (module C) are indicated separately.
instructions
Usage conditions, e.g. Use in areas defined by Recycling in the cement industry (scenario 3) Theorganic
frequency of use, mechanical the use class according - material of the carpet is used as an alternative fuel in a cement
exposure to EN 1307 kiln. It mainly substitutes for lignite (68.8%), hard coal (23.6%)
Maintenance e.g. required According to the and petrol coke (7.6%). The inorganic material is substantially
frequency, type and quality and manufacturers - integrated into the cement clinker and substitutes for original
replacement of components instructions material input. VDZ e.V.
4 Environmental Product Declaration - Interface - Tufted tiles, 100% recycled Polyamid 6 with a maximum total pile weight of 1500 g/m2, a CQuest Bio Sone+ backing
LCA: Results
The LCA results refer to all declared products with a maximum total pile weight of 1500 g/m2. LCA results for products with a maximum
total pile weight of 535 g/m2 can be taken from the corresponding tables of the annexe. Results for specific products with any other
total pile weight can be calculated by using equation 1 given in the annexe (see annexe chapter: 'General Information on the annexe').
The declared result figures in module B2 have to be multiplied by the assumed service life (in years) of the floor covering in the building
under consideration. Information on non-relevant modules: Modules B3 - B7 are not relevant during the service life of the carpet.
Modules C1, C3/1, C4/2 and C4/3 cause no additional impact (see chapter "LCA: Calculation rules" in this document). All these
modules are declared and marked as 'modules not relevant/declared'. Module C2 represents the transport for scenarios 1, 2 and 3.
Column D represents benefits from module A5 assembly.
DESCRIPTION OF THE SYSTEM BOUNDARY (X = INCLUDED IN LCA; ND = MODULE OR INDICATOR NOT DECLARED; MNR =
MODULE NOT RELEVANT)
Benefits and
Construction loads beyond
Product stage Use stage End of life stage
process stage the system
boundaries
la ire ta m w a Ry lp p u s tro p s n a rT g n iru tc a fu n a M e h t m o rf tro p s n a rTe tis e h t o t e ta g y lb m e s s A e s U e c n a n e tn ia M ria p e R tn e m e c a lp e R tn e m h s ib ru fe R y g re n e la n o ita re p Oe s u re ta w la n o ita re p Oe s u n o itc u rts n o c -e Dn o itilo m e d tro p s n a rT g n is s e c o rp e ts a W la s o p s iD -e s u e R-y re v o c e R-g n ilc y c e Rla itn e to p
A1 A2 A3 A4 A5 B1 B2 B3 B4 B5 B6 B7 C1 C2 C3 C4 D
X X X X X X X MNR MNR MNR MND MND X X X X X
RESULTS OF THE LCA - ENVIRONMENTAL IMPACT according to EN 15804+A2: 1 m² floor covering
Parameter Unit A1-A3 A4 A5 B1 B2 C1 C2 C3/2 C3/3 C4/1 D D/1 D/2 D/3
GWP-total kg CO 2 eq 5.45E+00 3.22E-01 4.83E-01 0 4.16E-01 0 1.8E-02 7.48E+007.55E+00 1.32E+00 -2.16E-02 0 -2.65E-01 -1.8E-01
GWP-fossil kg CO 2 eq 6.73E+00 3.16E-01 4.65E-01 0 2.15E-01 0 1.76E-02 6.53E+00 6.6E+00 3.71E-01 -2.15E-02 0 -2.64E-01 -1.8E-01
GWP- -1.29E
biogenic kg CO 2 eq +00 4.09E-03 1.71E-02 0 4.16E-03 0 2.28E-04 9.49E-01 9.5E-01 9.48E-01 -1.1E-04 0 -1.33E-03 -3.19E-04
GWP-luluc kg CO 2 eq 1.23E-02 1.79E-03 4.34E-04 0 1.96E-01 0 9.99E-05 2.3E-04 4.86E-04 1.83E-04 -2.35E-06 0 -2.84E-05 -8.85E-05
kg CFC11
ODP 2.86E-08 1.93E-14 8.59E-10 0 3.42E-08 0 1.07E-15 6.12E-13 1.01E-12 5.04E-13 -1.45E-13 0 -1.74E-12 -2.15E-13
eq
AP mol H+ eq 2.79E-02 1.91E-03 1.12E-03 0 8.32E-04 0 1.07E-04 7.11E-03 7.43E-03 1.11E-03 -2.82E-05 0 -3.42E-04 -7.12E-04
EP-
kg P eq 1.54E-04 9.59E-07 4.69E-06 0 5.19E-06 0 5.35E-08 8.61E-07 1.07E-06 7E-05 -2.94E-08 0 -3.54E-07 -1.96E-07
freshwater
EP-marine kg N eq 9.38E-03 9.39E-04 4.18E-04 0 1.97E-04 0 5.24E-05 3.51E-03 3.65E-03 2.46E-04 -7.66E-06 0 -9.34E-05 -2.11E-04
EP-terrestrial mol N eq 8.85E-02 1.04E-02 4.18E-03 0 2.83E-03 0 5.8E-04 3.92E-02 4.08E-02 2.7E-03 -8.21E-05 0 -1E-03 -2.31E-03
kg
POCP NMVOC 2.23E-02 1.78E-03 9.98E-04 4.18E-04 9.83E-04 0 9.9E-05 8.99E-03 9.27E-03 7.91E-04 -2.14E-05 0 -2.62E-04 -6.28E-04
eq
ADPE kg Sb eq 2.72E-06 2.69E-08 8.34E-08 0 2.3E-07 0 1.5E-09 3.11E-08 4.22E-08 2.6E-08 -3.23E-09 0 -3.91E-08 -1.75E-08
-4.48E -1.95E
ADPF MJ 1.02E+024.29E+00 3.3E+00 0 5.9E+00 0 2.4E-01 3.77E+004.86E+00 5.32E+00 -3.66E-01 0
+00 +01
m3 world
WDP eq 2.06E+01 2.87E-03 6.48E-01 0 9.99E-02 0 1.6E-04 9.15E-01 9.21E-01 -3.98E-03 -2.25E-03 0 -2.71E-02 -2.56E-02
deprived
GWP = Global warming potential; ODP = Depletion potential of the stratospheric ozone layer; AP = Acidification potential of land and water; EP =
Eutrophication potential; POCP = Formation potential of tropospheric ozone photochemical oxidants; ADPE = Abiotic depletion potential for non-fossil
resources; ADPF = Abiotic depletion potential for fossil resources; WDP = Water (user) deprivation potential)
RESULTS OF THE LCA - INDICATORS TO DESCRIBE RESOURCE USE according to EN 15804+A2: 1 m² floor covering
Parameter Unit A1-A3 A4 A5 B1 B2 C1 C2 C3/2 C3/3 C4/1 D D/1 D/2 D/3
PERE MJ 9.28E+01 2.44E-01 3.48E+00 0 3.69E+00 0 1.36E-02 1.41E+01 1.44E+01 4.38E-01 -9.99E-02 0 -1.2E+00 -2.66E-01
-1.34E -1.34E
PERM MJ 1.37E+01 0 -2.6E-01 0 0 0 0 0 0 0 0 0
+01 +01
PERT MJ 1.07E+02 2.44E-01 3.22E+00 0 3.69E+00 0 1.36E-02 6.18E-01 9.25E-01 4.38E-01 -9.99E-02 0 -1.2E+00 -2.66E-01
PENRE MJ 9.35E+01 4.3E+00 3.7E+00 0 5.9E+00 0 2.4E-01 1.15E+01 1.26E+01 5.33E+00 -3.66E-01 0 -4.49E+00-1.95E+01
-7.69E -7.69E
PENRM MJ 8.09E+00 0 -3.96E-01 0 0 0 0 0 0 0 0 0
+00 +00
PENRT MJ 1.02E+02 4.3E+00 3.3E+00 0 5.9E+00 0 2.4E-01 3.77E+00 4.86E+00 5.33E+00 -3.66E-01 0 -4.49E+00-1.95E+01
SM kg 4.58E+00 0 1.37E-01 0 0 0 0 0 0 0 0 0 0 1.5E-01
RSF MJ 0 0 0 0 0 0 0 0 0 0 0 0 0 0
NRSF MJ 0 0 0 0 0 0 0 0 0 0 0 0 0 0
FW m3 4.93E-01 2.76E-04 1.55E-02 0 3.34E-03 0 1.54E-05 2.16E-02 2.19E-02 6.24E-05 -9.54E-05 0 -1.15E-03 -1.86E-03
PERE = Use of renewable primary energy excluding renewable primary energy resources used as raw materials; PERM = Use of renewable primary
energy resources used as raw materials; PERT = Total use of renewable primary energy resources; PENRE = Use of non-renewable primary energy
excluding non-renewable primary energy resources used as raw materials; PENRM = Use of non-renewable primary energy resources used as raw
materials; PENRT = Total use of non-renewable primary energy resources; SM = Use of secondary material; RSF = Use of renewable secondary fuels;
5 Environmental Product Declaration - Interface - Tufted tiles, 100% recycled Polyamid 6 with a maximum total pile weight of 1500 g/m2, a CQuest Bio Sone+ backing
NRSF = Use of non-renewable secondary fuels; FW = Use of net fresh water
RESULTS OF THE LCA – WASTE CATEGORIES AND OUTPUT FLOWS according to EN 15804+A2:
1 m² floor covering
Parameter Unit A1-A3 A4 A5 B1 B2 C1 C2 C3/2 C3/3 C4/1 D D/1 D/2 D/3
HWD kg 4.24E-03 2.06E-11 1.27E-04 0 4.19E-05 0 1.15E-12 5.71E-10 6.16E-10 8.21E-10 -4.96E-11 0 -6.13E-10 -1.62E-10
NHWD kg 7.13E-01 6.17E-04 5.49E-02 0 7.3E-03 0 3.44E-05 1.11E+00 1.11E+00 5.27E+00 -1.84E-04 0 -2.24E-03 -9.82E-02
RWD kg 4.3E-03 5.3E-06 1.33E-04 0 3.76E-04 0 2.96E-07 1.35E-04 2.15E-04 6.54E-05 -2.86E-05 0 -3.44E-04 -5.89E-05
CRU kg 0 0 0 0 0 0 0 0 0 0 0 0 0 0
MFR kg 0 0 1.21E-01 0 0 0 0 0 1.25E+00 0 0 0 0 0
MER kg 0 0 0 0 0 0 0 0 0 0 0 0 0 0
EEE MJ 0 0 3.77E-01 0 0 0 0 1.05E+01 0 0 0 0 0 0
EET MJ 0 0 6.89E-01 0 0 0 0 1.93E+01 8.97E+01 0 0 0 0 0
HWD = Hazardous waste disposed; NHWD = Non-hazardous waste disposed; RWD = Radioactive waste disposed; CRU = Components for re-use;
MFR = Materials for recycling; MER = Materials for energy recovery; EEE = Exported electrical energy; EET = Exported thermal energy
RESULTS OF THE LCA – additional impact categories according to EN 15804+A2-optional:
1 m² floor covering
Parameter Unit A1-A3 A4 A5 B1 B2 C1 C2 C3/2 C3/3 C4/1 D D/1 D/2 D/3
Disease
PM 2.17E-07 1.11E-08 7.72E-09 0 6.84E-08 0 6.16E-10 2.8E-08 3E-08 1.07E-08 -2.34E-10 0 0 -9.98E-09
incidence
kBq U235
IR 7.06E-01 7.77E-04 2.19E-02 0 6.78E-02 0 4.33E-05 2.07E-02 3.42E-02 9.66E-03 -4.85E-03 0 0 -7.21E-03
eq
ETP-fw CTUe 1.11E+02 2.98E+00 3.48E+00 3.6E-03 2.69E+00 0 1.66E-01 1.74E+00 2.37E+00 5.21E+00 -7.98E-02 0 0 -3.59E+00
HTP-c CTUh 3.09E-09 6.03E-11 9.75E-11 0 6.21E-10 0 3.36E-12 8.95E-11 1.04E-10 2.34E-10 -3.68E-12 0 0 -4.95E-11
HTP-nc CTUh 8.65E-08 3.57E-09 2.89E-09 2.6E-11 9.46E-09 0 1.99E-10 5.63E-09 6.35E-09 1.96E-08 -1.42E-10 0 0 -3.14E-09
SQP SQP ND ND ND ND ND 0 6.11E-02 6.49E-01 9.33E-01 2.84E-01 ND ND ND ND
PM = Potential incidence of disease due to PM emissions; IR = Potential Human exposure efficiency relative to U235; ETP-fw = Potential comparative
Toxic Unit for ecosystems; HTP-c = Potential comparative Toxic Unit for humans (cancerogenic); HTP-nc = Potential comparative Toxic Unit for humans
(not cancerogenic); SQP = Potential soil quality index
No substantiated values can be given for the SQP indicator with the existing database.
The result figures given in module B2 refer to a period of 1 year because a reference service life is not declared. They have to be
multiplied by the assumed service life (in years) of the floor covering in the building under consideration.
Disclaimer 1 – for the indicator 'Potential Human exposure efficiency relative to U235'.
This impact category deals mainly with the eventual impact of low dose ionizingradiation on human health of the nuclear fuel cycle. It
does not consider effects due to possible nuclear accidents, occupational exposure nor due to radioactive waste disposal in
undergroundfacilities. Potential ionizing radiation from the soil, from radon and from some construction materials is also not measured
by this indicator.
Disclaimer 2 – for the indicators 'abiotic depletion potential for non-fossil resources', 'abiotic depletion potential for fossil resources',
'water (user) deprivation potential, deprivation-weighted water consumption', 'potential comparative toxic unit for ecosystems', 'potential
comparative toxic unit for humans – cancerogenic', 'Potential comparative toxic unit for humans - not cancerogenic', 'potential soil
quality index'.
The results of this environmental impact indicator shall be used with care as the uncertainties on these results are high or as there is
limited experienced with the indicator.
References
EN 1307 EN 16810
DIN EN 1307: 2014+A1:2016+A2:2018-05: Textile floor DIN EN 16810: 2017-08: Resilient, textile and laminate floor
coverings - Classification coverings – Environmental product declarations – Product
category rules
EN 13501-1
DIN EN 13501-1:2019-05: Fire classification of construction ISO 10874
products and building elements - Part 1: Classification using DIN EN ISO 10874: 2012+A1:2021-04: Resilient, textile and
data from reaction to fire tests laminate floor coverings - Classification
EN 14041 ISO 14025
DIN EN 14041: 2018-05 and DIN EN 14041: 2008-05: DIN EN /ISO 14025:2011-10/, Environmental labels and
Resilient, textile and laminate floor coverings - Essential declarations — Type III environmental declarations —
characteristics Principles and procedures
EN 15804 ISO 14040 DIN EN ISO 14040:2006+A1:2020 Environmental
DIN EN 15804:2012+A2:2019 + AC:2021, Sustainability of management - Life cycle assessment - Principles and
construction works — Environmental Product Declarations — framework
Core rules for the product category of construction products
ISO 14044 DIN EN ISO 14044:2006+A1:2018+A2:2020
6 Environmental Product Declaration - Interface - Tufted tiles, 100% recycled Polyamid 6 with a maximum total pile weight of 1500 g/m2, a CQuest Bio Sone+ backing
Environmental management - Life cycle assessment - September 2020
Requirements and guidelines
GaBi database
ISO 15686 GaBi Software-System and Database for Life Cycle
ISO 15686: Buildings and constructed assets - Service life Engineering, version 10.5 Sphera, Leinfelden-Echterdingen,
planning ISO 15686-1: 2011-05: Part 1: General principles and database version 2022-1
framework ISO 15686-2: 2012-05: Part 2: Service life prediction
procedures ISO 15686-7: 2017-04: Part 7: Performance PCR Part A
evaluation for feedback of service life data from practice ISO Product Category Rules for Building-Related Products and
15686-8: 2008-06: Part 8: Reference service life and service- Services Part A: Calculation Rules for the Life Cycle
life estimation Assessment and Requirements on the Project Report according
to EN 15804+A2:2019, V1.2, Berlin: Institut Bauen und Umwelt
Regulation (EU) No. 305/2011 e.V. (IBU), November 2021
Regulation No. 305/2011 Construction Products Regulation
(CPR) of the European Council and of the European PCR Part B
Parliament, April 2011 Product Category Rules for Building-Related Products and
Services Part B: Requirements on the EPD for floor coverings,
General Instructions for the IBU-EPD Program V1.2, Berlin: Institut Bauen und Umwelt e.V. (IBU), February
General Instructions for the EPD-Program of the Institut Bauen 2018
und Umwelt e.V., The Preparation of Environmental Product
Declarations - EPDs, version 2.0, Institut Bauen und Umwelt PRODIS
e.V., Berlin, January 2021, www.ibu-epd.de Product Information System (PRODIS) of the European Carpet
Industry, Gemeinschaft umweltfreundlicher Teppichboden e.V
BNB, Nutzungsdauer von Bauteilen (GUT) and European Carpet and Rug Association (ECRA),
Bewertungssystem Nachhaltiges Bauen (BNB), Nutzungsdauer http://www.pro-dis.info
von Bauteilen, Bundesministerium des Inneren, für Bau und
Heimat, 24.02.2017 REACH
Regulation (EC) No 1907/2006 of the European Parliament and
ECHA candidate list of the Council of 18 December 2006 concerning the
Candidate List of substances of very high concern (SVHCs) for Registration, Evaluation, Authorisation and Restriction of
authorisation, 08.07.2021, European Chemicals Agency Chemicals (REACH), June 2017, last update: 08.07.2021
(ECHA), Helsinki, Finland
VDZ e.V.
ecoinvent Association of German Cement Works, Ed. Environ-mental
ecoinvent, Zurich, Switzerland, database version 3.7, published Data of the German Cement Industry 2020
7 Environmental Product Declaration - Interface - Tufted tiles, 100% recycled Polyamid 6 with a maximum total pile weight of 1500 g/m2, a CQuest Bio Sone+ backing
Publisher
Institut Bauen und Umwelt e.V. +49 (0)30 3087748- 0
Hegelplatz 1 info@ibu-epd.com
10117 Berlin www.ibu-epd.com
Germany
Programme holder
Institut Bauen und Umwelt e.V. +49 (0)30 3087748- 0
Hegelplatz 1 info@ibu-epd.com
10117 Berlin www.ibu-epd.com
Germany
Author of the Life Cycle Assessment
Gemeinschaft umweltfreundlicher Teppichboden +49 (0)241 96843 410
(GUT) e.V. mail@gut-ev.de
Schönebergstraße 2 www.gut-ev.org
52068 Aachen
Germany
Owner of the Declaration
Interface Europe Manufacturing BV +31 33 277 55 55
Industrielaan 15 receptie@interface.com
3925ZG Scherpenzeel www.interface.com
Netherlands
8 Environmental Product Declaration - Interface - Tufted tiles, 100% recycled Polyamid 6 with a maximum total pile weight of 1500 g/m2, a CQuest Bio Sone+ backing
