ENVIRONMENTAL PRODUCT DECLARATION
as per ISO 14025 and EN 15804+A2
Owner of the Declaration
Programme holder Institut Bauen und Umwelt e.V. (IBU)
Publisher Institut Bauen und Umwelt e.V. (IBU)
Declaration number EPD-KNB-20210240-CBC1-EN
Issue date 21.03.2022
Valid to 20.03.2027
Gypsum plasters Bulgips Start, MP75, MP75 L, MP75 SL
and Rotband
Knauf Radika AD Debar
www.ibu-epd.com | https://epd-online.com
Umwelt Produktdeklaration Name des Herstellers – Name des Produkts
General Information
Knauf Radika AD Gypsum plasters Bulgips Start, MP75,
MP75 L, MP75 SL and Rotband
Programme holder Owner of the declaration
IBU – Institut Bauen und Umwelt e.V. Knauf Radika AD
Panoramastr. 1 8-mi Septemvri bb
10178 Berlin 1250 Debar
Germany Republic of North Macedonia
Declaration number Declared product / declared unit
EPD-KNB-20210240-CBC1-EN 1 kg gypsum plaster dry mix
This declaration is based on the product Scope:
category rules: This EPD represents the weighted average of the
Mineral factory-made mortar, 11.2017 following five gypsum plaster dry mix products:
(PCR checked and approved by the SVR) - Bulgips Start;
- MP75;
Issue date - MP75 L;
21.03.2022 - MP75 SL;
- ROTBAND.
Valid to
20.03.2027
All plasters are manufactured by:
Knauf Radika AD,
8-mi Septemvri bb
1250 Debar,
Republic of North Macedonia.
The LCA considers specific information provided by the
manufacturer and suppliers of components exclusively
for the cradle-to-gate production stage. The end-of-life
stage is modelled based on a developed scenario.
The owner of the declaration shall be liable for the
underlying information and evidence; the IBU shall not
be liable with respect to manufacturer information, life
cycle assessment data and evidences.
The EPD was created according to the specifications
of EN 15804+A2. In the following, the standard will be
simplified as EN 15804.
Verification
The standard EN 15804 serves as the core PCR
Independent verification of the declaration and data
according to ISO 14025:2010
Dipl. Ing. Hans Peters internally x externally
(chairman of Institut Bauen und Umwelt e.V.)
Dr. Alexander Röder Matthias Klingler
(Managing Director Institut Bauen und Umwelt e.V.)) (Independent verifier)
Product
Product description/Product definition dry mix product with weighted average density of 870
Knauf gypsum plasters are factory-made pre-mixed dry kg/m3.
gypsum plasters produced in accordance with EN The following products are included in this EPD:
13279. All declared plasters consist of mineral binders - Bulgips Start;
(mainly natural gypsum and hydrated lime in a small - MP75;
amount), fillers and additives. The declaration refers to - MP75 L;
the declared unit of 1 kg of an average gypsum plaster - MP75 SL;
- ROTBAND.
2 Environmental Product Declaration KNAUF Gipsputz: Bulgips Start, MP75, MP75 L, MP75 SL und Rotband – Gypsum
plasters Bulgips Start, MP75, MP75 L, MP75 SL and Rotband
Constructional data
For the placing on the market of the product in Name Value Unit
the European Union/European Free Trade Association Gross density 730-1000 kg/m3
(EU/EFTA) (with the exception of Switzerland) Surface hardness >5.0 N/mm2
Regulation (EU) No. 305/2011 (CPR) applies. The Compressive strength 2 N/mm2
product needs a declaration of performance taking into Flexural strength 1 N/mm2
consideration EN 13279-1:2008 Gypsum binders and Thermal conductivity 0.25 - 0.35 W/(mK)
gypsum plasters - Part 1: Definitions and Water vapour diffusion resistance
requirements and the CE-marking. For the application factor - µ (dry/wet) 10/6
and use the respective national provisions apply.
Application Regulation (EU) No.305/2011 applies for placing of the
The specific recommended applications of the declared products on the market within European
products are as follows: union/European Free Trade Association (EU/EFTA).
- Bulgips Start: intended for indoor machine KNAUF gypsum plasters are required to have
application as two-layer plaster in various residential declarations of performance and CE marking.
building systems (hotels, hospitals, administrative
premises), including premises with normal air humidity Base materials/Ancillary materials
acc. to DIN 18550-1 and DIN 18550-2. Bulgips Start The primary constituents of the gypsum plasters are
can be applied on walls and ceilings on various natural gypsum (70 % on a weighted average, varying
substrates: porous concrete, silicate masonry units, between 60 % and 90 %) and limestone filler (26 % on
pumice, concrete masonry, mixed masonry, gypsum a weighted average, varying between 5 % and 37 %).
fibreboards or stone walls. In addition, expanded perlite (<3 % on average),
- MP75, MP75 L and MP75 SL: intended for indoor hydrated lime (<1.5 % on average) and modifying
machine application to create smooth surfaces on additives (<1 %) are included in the mix.
walls and ceilings. It can be applied in one layer on all
types of masonry, concrete and stable plasterable This product contains the following substances listed in
foundations; in all premises with normal humidity, incl. the candidate list (date: 24.06.2021) exceeding 0.1
domestic kitchens and bathrooms; as a base for percentage by mass:
subsequent finishing or wallpapers, as a basis for tiles - Calcium dihydroxide, CAS No. 1305-62-0 (<1.5 %).
and finishing plasters.
- ROTBAND: intended for indoor manual application to Reference service life
be used on concrete slabs, walls, pre-cast concrete No reference service life is determined in accordance
elements and on all plasterable substrates. The with EN ISO 15686-1:2011. A service life of >50 years
product can be used in humid premises (kitchens, can be considered for the gypsum plasters in
bathrooms) acc. to DIN V 18550. accordance with the Bundesinstitut für Bau-, Stadt-
und Raumforschung (BBSR) table "Service lives of
components for life cycle assessment according to
Technical Data BNB".
The following technical information based on DoPs of
the delivered products is relevant for the declared
products:
LCA: Calculation rules
Declared Unit
The declared unit is 1 kg of KNAUF gypsum plaster as The data on supply of raw materials and production
an average of KNAUF gypsum plaster Bulgips Start, process is provided by Knauf Radika AD, so processes
MP75, MP75 L, MP75 SL and ROTBAND. with the highest contributions are representative for the
geographical conditions at the manufacturing plant.
Declared unit Where information is unavailable or unknown, it is
Name Value Unit modelled with background datasets preferably for the
Declared unit 1 kg European context
Gross density 870 kg/m3
The impact results represent the production of a
weighted average gypsum plaster. The products System boundary
included in the declaration use the same raw materials This EPD covers the production stage, the end-of-life
and the same production technology, so the variance stage and module D in accordance with EN 15804, i.e.
of results comes only from the different proportions of the scope is cradle-to-gate with options. The
ingredients. For Bulgips Start and MP75 the impacts production stage (modules A1-A3) includes the
are by 5 % smaller than declared weighted average production of raw materials and their transport to the
values for most indicators except for GWP-luluc, manufacturing site, production processes, packaging
ADPE, EP-terrestrial, ODP and POCP where the and the preparation for delivery, as well as the use of
variance is less than 10 %. For MP75 L and electricity, fuels and water. The end-of-life stage
ROTBAND the variance is within 1-2 % on all (modules C1-C4) includes the processes of
indicators. The impacts of MP75 SL are between 10 % dismantling/demolition of the building, transport of
and 15 % higher than the declared results. The highest gypsum plaster waste, waste processing and disposal.
variance is on ADPE, so this indicator should be
handled with care.
3 Environmental Product Declaration KNAUF Gipsputz: Bulgips Start, MP75, MP75 L, MP75 SL und Rotband – Gypsum
plasters Bulgips Start, MP75, MP75 L, MP75 SL and Rotband
Comparability context, respectively the product-specific
Basically, a comparison or an evaluation of EPD data characteristics of performance, are taken into account.
is only possible if all the data sets to be compared
were created according to EN 15804 and the building To model the LCA of the plasters, the ecoinvent
v3.7.1 database is used for background data.
LCA: Scenarios and additional technical information
Characteristic product properties the rest contribute to the C&DW coming from of the
Information on biogenic Carbon substrate material.
The biogenic carbon content is calculated for the
product itself and herein the weighted average values Name Value Unit
is declared (<0.2 %). The biogenic carbon content from Collected separately EWC 17 08
0.75 kg
packaging is calculated from the associated mass of 02
paper packaging and wooden pallets. Collected as mixed construction
waste EWC 17 01 01 and/or 17 0.25 kg
Information on describing the biogenic Carbon 01 02
Content at factory gate Landfilling 1 kg
Name Value Unit
Biogenic Carbon Content in Reuse, recovery and/or recycling potentials (D),
0.0012 kg C
product relevant scenario information
Module A5 is not declared, so the biogenic carbon of There are no available practices for use of the waste
the packaging is not included in the results of A1-A3. gypsum from gypsum plasters in Republic of North
Macedonia at the present moment, so this material
This declaration covers the product stage and the end- cannot be linked to other systems using gypsum. This
of-life stage of the gypsum plasters and does not is why, zero impacts for module D are assumed.
provide information about the installation and use
stages of the building.
Additional information for module A5 is provided below
regarding the accompanying packaging of the plasters.
Installation into the building (A5)
Additional technical scenario information on the
amount of packaging materials:
All plasters are packed in paper bags of 30 kg except
for MP75 SL, which is packed in bags of 25 kg. The
mass of each paper bag varies slightly, but on average
the paper packaging is 4.4 g per 1 kg gypsum plaster.
Plasters are packed on pallets and covered by PE foil
and the mass of the foil is 0.62 g per 1 kg plaster.
The usual mass on a pallet is 1050 kg for Bulgips
Start, MP75, MP75 L and ROTBAND, and 1000 kg for
MP74 SL. The wooden material associated with 1 kg of
plaster is on average 24 g per 1 kg plaster.
Name Value Unit
Mass of packaging per 1 kg
29 g
plaster
Reference service life
The service life of the gypsum plasters is declared in
accordance with BNB.
Name Value Unit
Life Span (according to BBSR) 50 a
Life Span according to the
50 a
manufacturer
End of life (C1-C4)
The deconstruction/demolition of the
plastered/rendered walls with gypsum plaster is
considered as a part of the entire demolition process of
the whole building. There are no specific
demolition/deconstruction methods, applied in
Republic of North Macedonia, with regards to the
gypsum plasters, because during the demolition
process the major share of plaster is self-detached and
4 Environmental Product Declaration KNAUF Gipsputz: Bulgips Start, MP75, MP75 L, MP75 SL und Rotband – Gypsum
plasters Bulgips Start, MP75, MP75 L, MP75 SL and Rotband
LCA: Results
Disclaimer:
EP-freshwater: This indicator has been calculated as “kg P eq” as required in the characterization model
(EUTREND model, Struijs et al., 2009b, as implemented in ReCiPe;
http://eplca.jrc.ec.europa.eu/LCDN/developerEF.xhtml).
DESCRIPTION OF THE SYSTEM BOUNDARY (X = INCLUDED IN LCA; ND = MODULE OR INDICATOR NOT
DECLARED; MNR = MODULE NOT RELEVANT)
BENEFITS AND
CONSTRUCTI LOADS
PRODUCT STAGE ON PROCESS USE STAGE END OF LIFE STAGE BEYOND THE
STAGE SYSTEM
BOUNDARIES
5 Environmental Product Declaration KNAUF Gipsputz: Bulgips Start, MP75, MP75 L, MP75 SL und Rotband – Gypsum
plasters Bulgips Start, MP75, MP75 L, MP75 SL and Rotband
lairetam
waR
ylppus tropsnarT
gnirutcafunaM
eht
morf
tropsnarT
etis
eht
ot
etag
ylbmessA esU
ecnanetniaM
riapeR
tnemecalpeR tnemhsibrufeR
ygrene
lanoitarepO esu
retaw
lanoitarepO esu
noitcurtsnoc-eD
noitilomed tropsnarT
gnissecorp
etsaW
lasopsiD -esueR -yrevoceR -gnilcyceR laitnetop
A1 A2 A3 A4 A5 B1 B2 B3 B4 B5 B6 B7 C1 C2 C3 C4 D
X X X ND ND ND ND MNR MNR MNR ND ND X X X X X
RESULTS OF THE LCA - ENVIRONMENTAL IMPACT according to EN 15804+A2: 1 kg gypsum plaster dry
mix (weighted average)
Core Indicator Unit A1-A3 C1 C2 C3 C4 D
Global warming potential - total [kg CO2-Eq.] 2.95E-1 0.00E+0 7.81E-3 7.50E-3 1.11E-1 0.00E+0
Global warming potential - fossil fuels [kg CO2-Eq.] 3.09E-1 0.00E+0 7.81E-3 7.49E-3 1.11E-3 0.00E+0
Global warming potential - biogenic [kg CO2-Eq.] -1.17E-3 0.00E+0 0.00E+0 9.00E-7 7.52E-8 0.00E+0
GWP from land use and land use change [kg CO2-Eq.] 4.50E-6 0.00E+0 5.73E-8 1.79E-8 2.59E-9 0.00E+0
Depletion potential of the stratospheric ozone layer [kg CFC11-Eq.] 6.93E-8 0.00E+0 1.72E-9 1.60E-9 2.38E-10 0.00E+0
Acidification potential, accumulated exceedance [mol H+-Eq.] 2.42E-3 0.00E+0 1.69E-5 1.30E-5 1.89E-6 0.00E+0
Eutrophication, fraction of nutrients reaching freshwater
[kg P-Eq.] 5.10E-4 0.00E+0 5.50E-7 3.40E-7 4.01E-8 0.00E+0
end compartment
Eutrophication, fraction of nutrients reaching marine end
[kg N-Eq.] 3.16E-4 0.00E+0 2.31E-6 1.76E-6 2.50E-7 0.00E+0
compartment
Eutrophication, accumulated exceedance [mol N-Eq.] 2.48E-3 0.00E+0 2.45E-5 1.88E-5 2.72E-6 0.00E+0
Formation potential of tropospheric ozone photochemical
[kg NMVOC-Eq.] 8.17E-4 0.00E+0 1.23E-5 1.03E-5 1.51E-6 0.00E+0
oxidants
Abiotic depletion potential for non-fossil resources [kg Sb-Eq.] 2.60E-5 0.00E+0 2.00E-7 1.15E-8 1.69E-9 0.00E+0
Abiotic depletion potential for fossil resources [MJ] 7.38E+0 0.00E+0 1.12E-1 1.01E-1 1.50E-2 0.00E+0
Water (user) deprivation potential, deprivation-weighted [m³ world-Eq
4.14E+1 0.00E+0 1.03E-1 4.47E-2 3.22E-3 0.00E+0
water consumption (WDP) deprived]
RESULTS OF THE LCA - INDICATORS TO DESCRIBE RESOURCE USE according to EN 15804+A2: 1 kg
gypsum plaster dry mix (weighted average)
Indicator Unit A1-A3 C1 C2 C3 C4 D
Renewable primary energy as energy carrier [MJ] 5.35E-1 0.00E+0 1.54E-3 8.14E-4 8.22E-5 0.00E+0
Renewable primary energy resources as material utilization [MJ] 1.26E-1 0.00E+0 0.00E+0 0.00E+0 0.00E+0 0.00E+0
Total use of renewable primary energy resources [MJ] 6.62E-1 0.00E+0 1.54E-3 8.14E-4 8.22E-5 0.00E+0
Non-renewable primary energy as energy carrier [MJ] 5.80E+0 0.00E+0 1.15E-1 1.03E-1 1.51E-2 0.00E+0
Non-renewable primary energy as material utilization [MJ] 2.00E+0 0.00E+0 0.00E+0 0.00E+0 0.00E+0 0.00E+0
Total use of non-renewable primary energy resources [MJ] 7.80E+0 0.00E+0 1.15E-1 1.03E-1 1.51E-2 0.00E+0
Use of secondary material [kg] 2.97E-3 0.00E+0 5.59E-5 5.11E-5 7.46E-6 0.00E+0
Use of renewable secondary fuels [MJ] 1.16E-2 0.00E+0 5.36E-5 3.61E-5 2.02E-6 0.00E+0
Use of non-renewable secondary fuels [MJ] 0.00E+0 0.00E+0 0.00E+0 0.00E+0 0.00E+0 0.00E+0
Use of net fresh water [m³] 3.53E-3 0.00E+0 7.75E-6 4.07E-6 4.20E-7 0.00E+0
RESULTS OF THE LCA – WASTE CATEGORIES AND OUTPUT FLOWS according to EN 15804+A2:
1 kg gypsum plaster dry mix (weighted average)
Indicator Unit A1-A3 C1 C2 C3 C4 D
Hazardous waste disposed [kg] 2.79E-3 0.00E+0 1.31E-4 1.15E-4 1.64E-5 0.00E+0
Non-hazardous waste disposed [kg] 1.70E-1 0.00E+0 5.62E-3 1.53E-3 1.75E-4 0.00E+0
Radioactive waste disposed [kg] 1.48E-5 0.00E+0 7.80E-7 7.20E-7 1.10E-7 0.00E+0
Components for re-use [kg] 0.00E+0 0.00E+0 0.00E+0 0.00E+0 0.00E+0 0.00E+0
Materials for recycling [kg] 4.00E-2 0.00E+0 0.00E+0 4.97E-5 7.33E-6 0.00E+0
Materials for energy recovery [kg] 1.20E-4 0.00E+0 0.00E+0 3.70E-7 2.27E-8 0.00E+0
Exported electrical energy [MJ] 0.00E+0 0.00E+0 0.00E+0 0.00E+0 0.00E+0 0.00E+0
Exported thermal energy [MJ] 0.00E+0 0.00E+0 0.00E+0 0.00E+0 0.00E+0 0.00E+0
RESULTS OF THE LCA – additional impact categories according to EN 15804+A2-optional:
1 kg gypsum plaster dry mix (weighted average)
Indicator Unit A1-A3 C1 C2 C3 C4 D
Potential incidence of disease due to PM emissions [Disease
8.66E-9 0.00E+0 1.60E-6 8.79E-7 4.25E-7 0.00E+0
Incidence]
Potential Human exposure efficiency relative to U235 [kBq U235-
2.92E-2 0.00E+0 1.82E+0 3.59E-1 5.78E-1 0.00E+0
Eq.]
Potential comparative toxic unit for ecosystems [CTUe] 2.74E-2 0.00E+0 1.21E+1 4.13E-1 2.47E+0 0.00E+0
Potential comparative toxic unit for humans - cancerogenic [CTUh] 8.37E-11 0.00E+0 7.16E-9 1.68E-9 3.47E-9 0.00E+0
Potential comparative toxic unit for humans - not cancerogenic [CTUh] 1.49E-8 0.00E+0 4.47E-7 8.14E-8 1.29E-7 0.00E+0
Potential soil quality index [-] 4.28E+0 0.00E+0 3.93E+2 4.28E+1 6.94E+1 0.00E+0
Disclaimer 1 – for the indicator “potential Human exposure efficiency relative to U235“.This impact category deals
mainly with the eventual impact of low dose ionizing radiation on human health of the nuclear fuel cycle. It does
not consider effects due to possible nuclear accidents, occupational exposure nor radioactive waste disposal in
underground facilities. Potential ionizing radiation from the soil, radon and (from) some construction materials is
also not measured by this indicator.
Disclaimer 2 – for the indicators: “abiotic depletion potential for fossil resources”, “abiotic depletion potential for
non-fossil resources”, “water (user) deprivation potential”, “deprivation-weighted water consumption”, “potential
comparative toxic unit for ecosystems”, “potential comparative toxic unit for humans - cancer effects”, “potential
comparative toxic unit for humans – non-cancer effects”, “potential soil quality index”. The results of this
environmental impact indicator shall be used with care as the uncertainties on these results are high or as there is
limited experience with the indicator.
References
Standards Buildings and constructed assets — Service life
planning — Part 1: General principles and framework
DIN 18550-1
DIN 18550-1 Putz und Putzsysteme - Ausführung EN 15804
EN 15804:2012+A2:2019 Sustainability of construction
works - Environmental product declarations - Core
DIN 18550-2 rules for the product category of construction products
DIN 18550-2 Planung, Zubereitung und Ausführung
von Außen- und Innenputzen - Teil 2: Ergänzende EN 15942
Festlegungen zu DIN EN 13914-2:2016-09 für EN 15942:2011, Sustainability of construction-
Innenputze Environmental product declarations. Communication
format business-to-business
DIN V 18550
DIN V 18550 Putz und Putzsysteme - Ausführung
Further References
EN ISO 10456
EN ISO 10456:2008 Building materials and products - BBSR
Hygrothermal properties -Tabulated design values and Nutzungsdauern von Bauteilen für
procedures for determining declared and design Lebenszyklusanalysen nach Bewertungssystem
thermal values (ISO 10456:2007) Nachhaltiges Bauen (BNB) – BBSR table "Service
lives of components for life cycle assessment
EN 13279-1 according to BNB" -
EN 13279-1:2008 Gypsum binders and gypsum https://www.nachhaltigesbauen.de/fileadmin/pdf/baust
plasters - Part 1: Definitions and requirements off_gebauededaten/BNB_Nutzungsdauern_von_Bautei
len_2017-02-24.pdf
BDS EN 13501-1
BDS EN 13501-1:2007+A1:2009 Fire classification of C&DW
construction products and building elements - Part 1: Construction and demolition waste
Classification using data from reaction to fire tests
DoP Bulgips Start
EN ISO 14025 Declaration of Performance No.
EN ISO 14025:2006, Environmental management – 0010_Bulgips_Start_2015-2-2 for gypsum plaster
Type III environmental declarations – Principles and Bulgips Start
procedure
DoP MP75
EN ISO 14040 Declaration of Performance No. 0010_MP75_2015 for
EN ISO 14040:2006, Environmental management -- gypsum plaster MP75
Life cycle assessment -- Principles and framework
DoP MP75 L
EN ISO 14044 Declaration of Performance No. 0010_MP75L_2015
EN ISO 14044:2006, Environmental management – for gypsum plaster MP75 L
Life cycle assessment – Requirements and guidelines
DoP MP75 SL
EN ISO 15686-1:2011
6 Environmental Product Declaration KNAUF Gipsputz: Bulgips Start, MP75, MP75 L, MP75 SL und Rotband – Gypsum
plasters Bulgips Start, MP75, MP75 L, MP75 SL and Rotband
Declaration of Performance No. 0093 IEA 2021
MP_75_SL_2014-01-23 for gypsum plaster MP75 SL International Energy Agency, www.iea.org (last visited
June 10, 2021)
DoP ROTBAND
Declaration of Performance No. Lab report 473/19
0010_ROTBAND_2015 for gypsum plaster ROTBAND Лабораториски Извештај бр. 473/19 од извршени
мерења на емисии во воздухот од “КНАУФ -
ECHA 2019 РАДИКА” АД Дебар, 2019 (Laboratory Report no.
Candidate List of substances of very high concern for 473/19 from performed measurements of air emissions
Authorisation, editor: European Chemicals Agency from "KNAUF - RADIKA" AD Debar), in Macedonian
(ECHA), Helsinki (FI), last update 25/02/2019,
https://echa.europa.eu/candidate-list-table Lab report 475/19
Лабораториски Извештај бр. 475/19 од извршени
ecoinvent анализи на отпадна вода од “КНАУФ - РАДИКА” АД
database ecoinvent v.3.7.1, The Ecoinvent Дебар, 2019 (Laboratory Report no. 475/19 from
Association, 2021 performed analyzes of wastewater from "KNAUF -
RADIKA" AD Debar), in Macedonian
ECRP 112
European Commission Radiation protection 112: openLCA
Radiological Protection Principles concerning the openLCA software for life cycle assessment, v. 1.10.2
Natural Radioactivity of Building Materials, 1999
Regulation 305
EWC 17 01 01 Regulation (EU) No 305/2011 of the European
EWC 17 01 01 Concrete Parliament and of the Council of 9 March 2011 laying
down harmnised conditions for the marketing of
EWC 17 01 02 construction products and repealing Council Directive
EWC 17 01 02 Bricks 89/106/EEC
EWC 17 08 02 Scherer
EWC 17 08 02 Gypsum-based construction materials Fraunhofer-Institut für Bauphysik IBP, Holzkirchen
other than those mentioned in 17 08 01 Prüfbericht Querschnittsuntersuchung zum
Emissionspotenzial an flüchtigen organischen
Gehrcke Verbindungen von Gipsbauteilen und Gipsprodukten
Gehrcke, K.; Hoffmann, B.; Schkade, U.; Schmidt, V.; des Wohninnenraums (Juli 2010) Veröffentlicht auf:
Wichterey, K; Natürliche Radioaktivität in www.gips.de (Rubrik: Forschungsvereinigung,
Baumaterialien und die daraus resultierende Projekte, 2010)
Strahlenexposition Fachbereich Strahlenschutz und
Umwelt, Bundesamt für Strahlenschutz Salzgitter, SDS Bulgips Start
November 2012, Data safety sheet for gypsum plaster Bulgips Start v.1
http://doris.bfs.de/jspui/bitstream/urn:nbn:de:0221- – 05.05.2017
201210099810/3/BfS_2012_SW_14_12.pdf
SDS MP75
IBU 2018 Data safety sheet for gypsum plaster MP75 v.1 –
IBU Product Category Rules (PCR) for Building- 05.05.2017
Related Products and Services Part A: Calculation
Rules for the Life Cycle Assessment and SDS MP75 L
Requirements on the Project Report–v. 1.7 (IBU PCR Data safety sheet for gypsum plaster MP75 L v.1 –
Part A-v.1.7, March, 2018) 05.05.2017
IBU 2021 SDS MP75 SL
General Instructions for the EPD programme of Institut Data safety sheet for gypsum plaster MP75 SL v.1 –
Bauen und Umwelt e.V. Version 2.0, Berlin: Institut 05.05.2017
Bauen und Umwelt e.V., 2021. www.ibu-epd.com
SDS ROTBAND
IBU PCR Part B Safety data sheet for gypsum plaster ROTBAND v.1 –
IBU PCR Guidance-Texts for Building-Related 05.05.2017
Products and Services Part B: Requirements on the
EPD for Mineral factory-made mortar (IBU PCR Part B:
Mineral factory-made mortar v. 1.6, 30.11.2017)
7 Environmental Product Declaration KNAUF Gipsputz: Bulgips Start, MP75, MP75 L, MP75 SL und Rotband – Gypsum
plasters Bulgips Start, MP75, MP75 L, MP75 SL and Rotband
Publisher
Institut Bauen und Umwelt e.V. Tel +49 (0)30 3087748- 0
Panoramastr. 1 Fax +49 (0)30 3087748- 29
10178 Berlin Mail info@ibu-epd.com
Germany Web www.ibu-epd.com
Programme holder
Institut Bauen und Umwelt e.V. Tel +49 (0)30 - 3087748- 0
Panoramastr 1 Fax +49 (0)30 – 3087748 - 29
10178 Berlin Mail info@ibu-epd.com
Germany Web www.ibu-epd.com
Author of the Life Cycle
Assessment Tel +359878622367
Green ReStart OOD Fax No fax
Shipchenski prohod Blvd., entr. V, Mail office@greenrestart.com
office 8 65 Web www.greenrestart.com
1574 Sofia
Bulgaria
Owner of the Declaration
Knauf Radika AD Tel +38946839-0
8-mi Septemvri bb - Fax +38946839-232
1250 Debar (Macedonia) Mail info@knauf.com.mk
(Others) Web www.knauf.com.mk
