ENVIRONMENTAL PRODUCT DECLARATION
as per ISO 14025 and EN 15804
Owner of the Declaration ArcelorMittal Europe - Flat Products
Programme holder Institut Bauen und Umwelt e.V. (IBU)
Publisher Institut Bauen und Umwelt e.V. (IBU)
Declaration number EPD-ARC-20200026-CBD1-EN
ECO EPD Ref. No. ECO-00001268
Issue date 10.07.2020
Valid to 09.07.2025
Hot Rolled Steel Coils
ArcelorMittal Europe
www.ibu-epd.com | https://epd-online.com
Umwelt Produktdeklaration Name des Herstellers – Name des Produkts
General Information
ArcelorMittal Europe Hot Rolled Steel Coils
Programme holder Owner of the declaration
IBU – Institut Bauen und Umwelt e.V. ArcelorMittal Europe – Flat Products
Panoramastr. 1 24-26 Boulevard d’Avranches
10178 Berlin L-1160 Luxembourg
Germany Luxembourg
Declaration number Declared product / declared unit
EPD-ARC-20200026-CBD1-EN The declared unit is 1 ton of hot rolled steel coil.
This declaration is based on the product Scope:
category rules: The Life Cycle Assessment is based on data collected
Structural steels, 07.2014 from the ArcelorMittal plants producing Hot Rolled
(PCR checked and approved by the SVR) Coils, representing 95% of the annual production from
2015.
Issue date
10.07.2020 The owner of the declaration shall be liable for the
underlying information and evidence; the IBU shall not
be liable with respect to manufacturer information, life
Valid to
cycle assessment data and evidences.
09.07.2025
Verification
The standard EN 15804 serves as the core PCR
Independent verification of the declaration and data
according to ISO 14025:2010
Dipl. Ing. Hans Peters internally x externally
(chairman of Institut Bauen und Umwelt e.V.)
Dr. Alexander Röder Mr Carl-Otto Neven
(Managing Director Institut Bauen und Umwelt e.V.)) (Independent verifier appointed by SVR)
Product
Product description/Product definition conditions. For the application and use the respective
This Environmental Product Declaration refers to Hot national provisions Apply.
Rolled Steel Coil, Slit Coil and Sheet, including
Indaten® weathering steel and Amstrong® high Other European standards concerning Hot Rolled Coils
strength steel range. The EPD results reflect the could also be used by manufacturers as reference:
volume weighted average of these products. EN 10149-1:2013 - Hot rolled flat products made of
high yield strength steels for cold-forming - Part 1:
Hot Rolled Coils are produced in ArcelorMittal hot- General technical delivery conditions can be
rolling mill in which solidified steel preheated to a high considered as specified in EN 1993-1-3:2006 -
temperature is continuously rolled between a series of Eurocode 3 - Design of steel structures - Part 1-3:
stands of rotating cylinders. Alloy composition and General rules - Supplementary rules for cold-formed
process parameters are set to guarantee the required members and sheeting. Products covered by EN
grade. The coils are then delivered to manufacturers 10149-1:2013 are not under CPR and did not request
for shaping into end products to be included in building CE marking to be placed on the market
works, generally to precise dimensions, thereby
avoiding losses on the construction site. Characteristics are also specified in the American
standard ASTM G101-04:2015 (American Society for
Mean thickness value is at 5 mm but the declaration Testing and Materials) for hot rolled material.
covers the whole range from 1.5 mm up to 25.4 mm.
Width range is from 45 mm up to 2150 mm.
Application
For the placing of the product on the market in the Hot Rolled Coils can be used in various construction
European Union/European Free Trade Association applications, such as:
(EU/EFTA) (with the exception of Switzerland)  Construction: structural or non-structural
Regulation (EU) No. 305/2011 (CPR) applies. The welded sections, façade & cladding, roofing,
product has a declaration of performance taking into
sun screens & shades.
consideration EN 10025-1:2004 - Hot rolled products
 Road equipment: safety barriers, protection
of structural steels - Part 1: General technical delivery
equipment, sound insulation wall panels.
2 Environmental Product Declaration ArcelorMittal – Hot rolled steel coil
 Art sculpture & Other industrial applications:
Containers & filters, etc. Base materials/Ancillary materials
The basic materials for the manufacture of
ArcelorMittal’s steel coil are non-alloyed and fine grain
steel. Different steel grades and qualities are possible,
Hot Rolled Coils are delivered in wide coils, slit coils or these being recorded in the specific product standards
cut-to-length sheets. It can be processed by all EN 10025-1:2004 and EN 10025-2:2019 or EN 10025-
conventional processing operations used for hot rolled: 3:2019 or EN 10025-4:2019 or EN 10025-5:2019 or
cutting and oxy-cutting, slitting, bending, drawing, EN 10149-1:2013 and EN 10149-2:2013 or EN 10149-
clinching, profiling, stamping, welding etc. 3:2013.
Indaten® weathering steels offer improved resistance Steel is mainly iron and carbon, with small amounts of
to corrosion thanks to the addition of copper during alloying elements. These elements modify the
manufacture. chemical and physical properties of steel such as
Additional alloying elements can be added to increase strength, durability and corrosion resistance. High
the steel’s tensile strength or make forming processes strength low alloyed (HSLA) carbon steel has a carbon
easier. content lower than 0.2 %.
When weathering steel is exposed to the ambient
atmosphere it develops an initial layer of iron oxide in The metallurgical composition of weathering steels
the same way as carbon steel. The rate of oxidation includes less than 0.2 % carbon. Alloying elements
depends on how much oxygen, moisture, and (mainly copper, chromium, nickel, phosphorus, silicon,
atmospheric contaminants can access the surface of and manganese) typically comprise less than 5% of
the metal. In the initial stages, a complex mix of iron the steel. Due to their specific chemistry, the corrosion
oxides covers the surface to create a layer of rust. As rate of weathering steels is generally much lower than
the process progresses, the rust layer forms a barrier that of standard carbon steel. The possible chemical
against the corrosive agents and the rate of corrosion compositions are defined in European standard.
slows down. Weathering steels can be classified into two
categories: those with limited phosphorous content
Amstrong® high-strength steels are available as (typically less than 0.035 %); and those with a higher
thermo-mechanically hot rolled, cold formable grades. phosphorous content. Weathering steels with a
Their main properties include high yield strength and phosphorous content of between 0.06 and 0.15 % are
tensile strength, combined with appropriate formability, identified by the letter P at the end of the product
toughness at low temperatures and fatigue resistance. name.
These grades are an excellent choice for reducing
structural thickness and weight whilst improving load- High levels of phosphorous improves the corrosion
bearing capacity. These grades have better ductility resistance of weathering steels. This can hamper
and bendability than standard high‑strength low‑alloy weldability and cause the weld zone to become brittle.
(HSLA) grades. For this reason, phosphorous weathering steels are
usually only available in thicknesses lower than 12
Technical Data mm.
ArcelorMittal Europe Flat products is producing Hot
Rolled Steel Coils in 8 mills. The EPD covers 95 % of This product contains substances listed in the
the total production in 2015. candidate list (date: 26.2.2020) exceeding 0.1
percentage by mass: no
ArcelorMittal offers a full range of grades in compliance
with the EN 10025-1 and EN 10025-2 or EN 10025-3 Reference service life
or EN 10025-4 or 10025-5 or EN 10149-1 and EN A reference service life for hot rolled steel coil is not
10149-2 or EN 10149-3 to meet different applications. declared. Hot rolled coil products are construction
Yield strengths from 235 MPa up to 700 MPa are products with many different application purposes. The
available. lifetime therefore will be limited by the application as
well as the service life of the work.
ArcelorMittal has also created different grades of
Indaten® weathering steels to meet different First structural steel projects using weathering steel
applications. Their chemical composition and were completed 50 years ago in Europe and have
mechanical performance are specified in EN 10025-5. demonstrated a very low maintenance level and no
need for painting.
Constructional data
Name Value Unit At the end of life, weathering steel products could be
Density 7850 kg/m3
recovered, recycled and sent to the steel mill.
Modulus of elasticity 210000 MPa
Melting point 1650 °C
Thermal conductivity 48 W/(mK)
Coefficient of thermal expansion 12 10-6K-1
Minimum yield strength 235 - 700 MPa
Performance data of the product in accordance with
the declaration of performance with respect to its
essential characteristics according to EN 10025-
1:2004 - Hot rolled products of structural steels - Part
1: General technical delivery conditions.
3 Environmental Product Declaration ArcelorMittal – Hot rolled steel coil
LCA: Calculation rules
Declared Unit · Production processes on-site including energy,
This Environmental Product Declaration refers to Hot production of additives, disposal of production
Rolled Steel Coil, Slit Coil and Sheet, including residues, and consideration of related emissions
Indaten® weathering steel and Amstrong® high · Recycling of production/manufacturing scrap. Steel
strength steel range, as specified in Part B scrap is assumed to reach the end-of-waste status
requirements on the EPD for Structural Steels. once it is shredded and sorted, thus becomes input to
the product system in the inventory.
Declared unit
Name Value Unit Module C3 takes into account the sorting and
Declared unit 1000 kg shredding of after-use steel that is recycled, as well as
Conversion factor to 1 kg 0.001 - the non-recovered scrap due to sorting efficiency
Density 7850 kg/m3 which is landfilled. A conservative value of 2 % landfill
is considered.
Module D refers to the End-of-Life of the steel coil,
System boundary including reuse and recycling.
Type of the EPD: cradle-to-gate - with options.
Module A1-A3, Module C3 and module D were Comparability
considered. Basically, a comparison or an evaluation of EPD data
is only possible if all the data sets to be compared
Modules A1-A3 of the Hot Rolled Steel Coil, Slit Coil were created according to EN 15804 and the building
and Sheet, including Indaten® weathering steel, and context, respectively the product-specific
Amstrong® high strength steel range production characteristics of performance, are taken into account.
include the following:
· The provision of resources, additives, and energy Gabi version 9.2 was used with Gabi Database SP35
· Transport of resources and additives to the version 8.7 to calculate this EPD.
production site
LCA: Scenarios and additional technical information
Current practice for the average Hot Rolled Steel Coil
consist of 98 % recycling and 2 % landfill according to
the European Commission Technical Steel Research.
End of life (C3)
Name Value Unit
Landfilling 2 %
Reuse, recovery and/or recycling potentials (D),
relevant scenario information
Name Value Unit
Recycling 98 %
4 Environmental Product Declaration ArcelorMittal – Hot rolled steel coil
LCA: Results
DESCRIPTION OF THE SYSTEM BOUNDARY (X = INCLUDED IN LCA; MND = MODULE NOT DECLARED;
MNR = MODULE NOT RELEVANT)
BENEFITS AND
CONSTRUCTI LOADS
PRODUCT STAGE ON PROCESS USE STAGE END OF LIFE STAGE BEYOND THE
STAGE SYSTEM
BOUNDARIES
5 Environmental Product Declaration ArcelorMittal – Hot rolled steel coil
lairetam
waR
ylppus tropsnarT
gnirutcafunaM
eht
morf
tropsnarT
etis
eht
ot
etag
ylbmessA esU
ecnanetniaM
riapeR
tnemecalpeR tnemhsibrufeR
ygrene
lanoitarepO esu
retaw
lanoitarepO esu
noitcurtsnoc-eD
noitilomed tropsnarT
gnissecorp
etsaW
lasopsiD -esueR -yrevoceR -gnilcyceR laitnetop
A1 A2 A3 A4 A5 B1 B2 B3 B4 B5 B6 B7 C1 C2 C3 C4 D
X X X MND MND MND MND MNR MNR MNR MND MND MND MND X MND X
RESULTS OF THE LCA - ENVIRONMENTAL IMPACT: 1 ton of hot rolled steel coil
Parameter Unit A1-A3 C3 D
Global warming potential [kg CO2-Eq.] 2.23E+3 2.00E+0 -1.64E+3
Depletion potential of the stratospheric ozone layer [kg CFC11-Eq.] 4.60E-9 6.89E-12 3.23E-10
Acidification potential of land and water [kg SO2-Eq.] 3.79E+0 6.78E-3 -3.96E+0
Eutrophication potential [kg (PO4)3--Eq.] 3.90E-1 7.99E-4 -3.39E-1
Formation potential of tropospheric ozone photochemical oxidants [kg ethene-Eq.] 6.70E-1 4.75E-4 -5.09E-1
Abiotic depletion potential for non-fossil resources [kg Sb-Eq.] 7.78E-5 9.53E-7 1.69E-4
Abiotic depletion potential for fossil resources [MJ] 1.91E+4 2.25E+1 -1.30E+4
RESULTS OF THE LCA - RESOURCE USE: 1 ton of hot rolled steel coil
Parameter Unit A1-A3 C3 D
Renewable primary energy as energy carrier [MJ] 2.95E+2 1.12E+1 1.19E+3
Renewable primary energy resources as material utilization [MJ] 0.00E+0 0.00E+0 0.00E+0
Total use of renewable primary energy resources [MJ] 2.95E+2 1.12E+1 1.19E+3
Non-renewable primary energy as energy carrier [MJ] 1.89E+4 3.43E+1 -1.23E+4
Non-renewable primary energy as material utilization [MJ] 0.00E+0 0.00E+0 0.00E+0
Total use of non-renewable primary energy resources [MJ] 1.89E+4 3.43E+1 -1.23E+4
Use of secondary material [kg] 1.18E+2 0.00E+0 0.00E+0
Use of renewable secondary fuels [MJ] 0.00E+0 0.00E+0 0.00E+0
Use of non-renewable secondary fuels [MJ] 0.00E+0 0.00E+0 0.00E+0
Use of net fresh water [m³] 3.84E+0 1.53E-2 5.76E-1
RESULTS OF THE LCA – OUTPUT FLOWS AND WASTE CATEGORIES:
1 ton of hot rolled steel coil
Parameter Unit A1-A3 C3 D
Hazardous waste disposed [kg] 1.29E-5 2.18E-7 -8.62E-6
Non-hazardous waste disposed [kg] 3.68E+0 2.01E+1 -2.61E+1
Radioactive waste disposed [kg] -6.70E-2 4.70E-3 2.93E-1
Components for re-use [kg] 0.00E+0 0.00E+0 0.00E+0
Materials for recycling [kg] 0.00E+0 9.80E+2 0.00E+0
Materials for energy recovery [kg] 0.00E+0 0.00E+0 0.00E+0
Exported electrical energy [MJ] 0.00E+0 0.00E+0 0.00E+0
Exported thermal energy [MJ] 0.00E+0 0.00E+0 0.00E+0
References
EN 10025-1 to 5 structural steels with improved atmospheric corrosion
EN 10025-1:2004 - Hot rolled products of structural resistance
steels - Part 1: General technical delivery conditions
EN 10025-2:2019 - Hot rolled products of structural EN 10149-1 to 3
steels - Part 2: Technical delivery conditions for non- EN 10149-1:2013 - Hot rolled flat products made of
alloy structural steels high yield strength steels for cold forming - Part 1:
EN 10025-3:2019 - Hot rolled products of structural General technical delivery conditions
steels - Part 3: Technical delivery conditions for EN 10149-2:2013 - Hot rolled flat products made of
normalized/normalized rolled weldable fine grain high yield strength steels for cold forming - Part 2:
structural steels Technical delivery conditions for thermomechanically
EN 10025-4:2019 - Hot rolled products of structural rolled steels
steels - Part 4: Technical delivery conditions for EN 10149-3:2013 - Hot rolled flat products made of
thermomechanical rolled weldable fine grain structural high yield strength steels for cold forming - Part 3:
steels Technical delivery conditions for normalized or
EN 10025-5:2019 - Hot rolled products of structural normalized rolled steels
steels - Part 5: Technical delivery conditions for
Declarations — Core rules for the product category of
EN 1993-1-3 construction products
EN 1993-1-3:2006 - Eurocode 3 - Design of steel
structures - Part 1-3: General rules - Supplementary European Commission Technical Steel Research
rules for cold-formed members and sheeting Sansom, M.and Meijer, J.:Life-cycle assessment (LCA)
for steel construction, European Commission technical
ASTM G101-04 steel research, 2001-12
ASTM G101-04:2015 - Standard Guide for Estimating
the Atmospheric Corrosion Resistance of Low-Alloy GaBi ts Software
Steels GaBi ts. Software and Databases
5 Environmental Product Declaration ArcelorMittal –
PCR Part B Organic coated steel coils Granite® and Estetic® for
PCR - Part B: Requirements of the EPD for Structural Life Cycle Engineering. LBP, University of Stuttgart
steels, und PE International, 2017.
Institut Bauen und Umwelt e.V., www.bauumwelt.com,
2017 GaBi ts Documentation
Documentation of the GaBi datasets for Life Cycle
Institut Bauen und Umwelt Engineering. LBP, Universitity of Stuttgart and PE
Institut Bauen und Umwelt e.V., Berlin (pub.): International, 2017.
Generation of Environmental Product Declarations http://documentation.gabi-software.com
(EPDs);
REACH
ISO 14025 Regulation (EC) No 1907/2006 of the European
DIN EN ISO 14025:2011-10 - Environmental labels Parliament and of the Council on the Registration,
and Evaluation, Authorisation and Restriction
declarations — Type III environmental declarations — of Chemicals (REACH)
Principles and procedures https://echa.europa.eu/regulations/reach/legislation
EN 15804
EN 15804:2012-04+A1:2013 - Sustainability of
construction works — Environmental Product
6 Environmental Product Declaration ArcelorMittal – Hot rolled steel coil
Publisher
Institut Bauen und Umwelt e.V. Tel +49 (0)30 3087748- 0
Panoramastr. 1 Fax +49 (0)30 3087748- 29
10178 Berlin Mail info@ibu-epd.com
Germany Web www.ibu-epd.com
Programme holder
Institut Bauen und Umwelt e.V. Tel +49 (0)30 - 3087748- 0
Panoramastr 1 Fax +49 (0)30 – 3087748 - 29
10178 Berlin Mail info@ibu-epd.com
Germany Web www.ibu-epd.com
Author of the Life Cycle
Assessment Tel +352 4792-1
ArcelorMittal Europe – Flat Products Fax -
Boulevard d’Avranches 24-26 Mail
1160 Luxembourg flateurope.technical.assistance
Luxembourg @arcelormittal.com
Web flateurope.arcelormittal.com/
Owner of the Declaration
ArcelorMittal Europe – Flat Products Tel +352 4792-1
Boulevard d’Avranches 24-26 Fax -
1160 Luxembourg Mail
Luxembourg flateurope.technical.assistance
@arcelormittal.com
Web flateurope.arcelormittal.com/
