ENVIRONMENTAL PRODUCT DECLARATION
as per ISO 14025 and EN 15804+A2
Owner of the Declaration Kermi GmbH
Publisher Institut Bauen und Umwelt e.V. (IBU)
Programme holder Institut Bauen und Umwelt e.V. (IBU)
Declaration number EPD-KER-20230254-CCB1-EN
Issue date 29.08.2023
Valid to 28.08.2028
Steel radiator
Kermi GmbH
www.ibu-epd.com | https://epd-online.com
General Information
Kermi GmbH Steel radiator
Programme holder Owner of the declaration
IBU – Institut Bauen und Umwelt e.V. Kermi GmbH
Hegelplatz 1 Pankofen-Bahnhof 1
10117 Berlin 94447 Plattling
Germany Germany
Declaration number Declared product / declared unit
EPD-KER-20230254-CCB1-EN The environmental product declaration refers to the declared unit of 1 kg
steel radiator.
This declaration is based on the product category rules: Scope:
Radiators, 24.07.2023 This document relates to the manufacture, transport, installation, operation
(PCR checked and approved by the SVR) and disposal of steel radiators. The products are produced in Germany
and the Czech Republic. The production data was collected at the
Pankofen plant and Stříbro in 2021.
Issue date
This EPD applies to the following product groups:
29.08.2023
• Steel panel radiators/plate radiators
• Heating walls/flat tube radiators
Valid to
28.08.2028 • Convectors/flat tube radiators
• Design radiators/round tube radiators
The owner of the declaration shall be liable for the underlying information
and evidence; the IBU shall not be liable with respect to manufacturer
information, life cycle assessment data and evidences.
The EPD was created according to the specifications of EN 15804+A2. In
the following, the standard will be simplified as EN 15804.
Verification
Dipl.-Ing. Hans Peters The standard EN 15804 serves as the core PCR
(Chairman of Institut Bauen und Umwelt e.V.)
Independent verification of the declaration and data according to ISO
14025:2011
internally X externally
Florian Pronold Mr Olivier Muller,
(Managing Director Institut Bauen und Umwelt e.V.) (Independent verifier)
1 Environmental Product Declaration - Kermi GmbH - Steel radiator
Product
Name Value Unit
Product description/Product definition
Heat output at room temperature 20 °C -
Steel radiators are parts of heating systems in buildings. As 88 - 8017 W
75/65 °C
heat exchangers, the hollow bodies made of steel release part
2.58 -
of the thermal energy transported by the heating medium Weight kg
252.3
(water) to the environment in order to increase the room
temperature. content of water 0.1 - 77.14 l
The heat is mainly transferred by conduction to the surrounding flow temperature max. 110 °C
air, which then distributes the heat in the room via natural working pressure max. 10 bar
convection (heat flow), as well as to varying degrees via
Paint type Powder -
thermal radiation.
How much heat a panel radiator gives off depends on the The performance values of the product according to the
temperature setting of the thermostats and how much water declaration of performance with regard to its essential
thus flows through it. characteristics in accordance with EN 442 'Radiators and
convectors”.
Further information can be found in the manufacturer's
Base materials/Ancillary materials
documentation. Regulation (EU) No 305/2011(CPR) applies to
the placing on the market of the product in the EU/EFTA The following table shows the percentage of basic
(excluding Switzerland). and auxiliary materials in steel radiators from the production
The required declarations of performance and CE marking have sites in
been prepared in accordance with the requirements of the Plattling and Stříbro.
harmonised standards EN 442-1:2014 Name Value Unit
'Radiators and convectors - Part 1: Technical specifications and BF Steel sheet 74.48 %
requirements' and EN 442-2:2014 'Radiators and convectors -
Steel pipes 23.29 %
Part 2: Test methods and performance specification'.
Epoxy-Polyester-Powder Coating 0.80 %
The respective national regulations apply to the use.
Cathodic / Anodic Dip Coating 0.68 %
Application Support inset 0.30 %
Steel radiators are used indoors for private or commercial use Korrolan 0.45 %
to increase the room temperature.
Technical Data
Reference service life
The products meet the requirements according to harmonised
regulations for CE marking, RAL-GZ 618 quality assurance and Steel radiators are durable products. When used properly, their
EN 442. average lifespan extends over
several decades. As a rule, steel radiators achieve a reference
Constructional Data
service life of at least 30 years, although a significantly longer
The following data refer to the entire steel radiator range. The service life is of course also possible.
exact data for each type can be found in the manufacturer's
documentation.
LCA: Calculation rules
packaging materials.
Declared Unit
The declared unit is 1 kg of Steel radiator. End of Life stage (C1-C4): The end of life (EoL) stage consists
Name Value Unit of:
Declared unit 1 kg - C1 Load free, manual deconstruction,
- C2 Transport of 50km to waste processing unit by truck,
By scaling the environmental indicators with respect to 1 kg of
- C3 Material recycling without expenses for separation and
radiator the LCA results of different product variations can be
sorting
approximated.
- C4 Not relevant
System boundary
Benefits and loads beyond the System Boundary (D):
Type of EPD: Cradle to gate (A1-A3, C1-C4, and module D)
Module D includes: Recovery from steel recycling, energy
with options (A4, A5):
recovery potentials from the electricity and thermal recycling of
the mixed plastic waste from packaging except for plastics.
Production Stage (A1-A3): The production stage includes:
- A1 Raw material supply and processing, Geographic Representativeness
- A2 Transport of raw materials to the manufacturer by truck,
Land or region, in which the declared product system is
- A3 Production of Steel radiator ( incl. energy provision, water
manufactured, used or handled at the end of the product´s
provision, disposal of production waste, production of
lifespan: Europe
packaging material)
Construction Stage (A4-A5): The stage of construction Comparability
includes: Basically, a comparison or an evaluation of EPD data is only
- A4 Transport to the construction site 100km by truck, possible if all the data sets to be compared were created
- A5 Load free manual installation, loads from the treatment of according to EN 15804 and the building context, respectively
2 Environmental Product Declaration - Kermi GmbH - Steel radiator
the product-specific characteristics of performance, are taken database
into account. The background data comes from the GaBi /GaBi software Version CUP2022.2
LCA: Scenarios and additional technical information
Installation into the building (A5)
Characteristic product properties of biogenic carbon
Module A5 includes installation of the product without machine
and the treatment and disposal of the packaging material.
Name Value Unit
Information on describing the biogenic Carbon Content at
factory gate Wooden Pallets 0.1321 kg
Cardboard 0.006 kg
Name Value Unit
Polyethylene 0,002 kg
kg
Biogenic carbon content in product -
C
End of life (C1-C4)
Biogenic carbon content in accompanying kg
0.0571 Name Value Unit
packaging C
Recycling 1 kg
Note: 1 kg of biogenic carbon is equivalent to 44/12 kg of CO .
2
Reuse, recovery and/or recycling potentials (D), relevant
scenario information
100% collection rate
Transport to the building site (A4)
Name Value Unit
Transport distance 100 km
3 Environmental Product Declaration - Kermi GmbH - Steel radiator
LCA: Results
DESCRIPTION OF THE SYSTEM BOUNDARY (X = INCLUDED IN LCA; MND = MODULE OR INDICATOR NOT DECLARED; MNR
= MODULE NOT RELEVANT)
Benefits and
Construction loads beyond
Product stage Use stage End of life stage
process stage the system
boundaries
la ire ta m w a Ry lp p u s tro p s n a rT g n iru tc a fu n a M e h t m o rf tro p s n a rTe tis e h t o t e ta g y lb m e s s A e s U e c n a n e tn ia M ria p e R tn e m e c a lp e R tn e m h s ib ru fe R y g re n e la n o ita re p Oe s u re ta w la n o ita re p Oe s u n o itc u rts n o c -e Dn o itilo m e d tro p s n a rT g n is s e c o rp e ts a W la s o p s iD -e s u e R-y re v o c e R-g n ilc y c e Rla itn e to p
A1 A2 A3 A4 A5 B1 B2 B3 B4 B5 B6 B7 C1 C2 C3 C4 D
X X X X X MND MND MNR MNR MNR MND MND X X X X X
RESULTS OF THE LCA - ENVIRONMENTAL IMPACT according to EN 15804+A2: 1 kilogram Steel radiator
Parameter Unit A1-A3 A4 A5 C1 C2 C3 C4 D
GWP-total kg CO 2 eq 2.66E+00 7.5E-03 2.16E-01 0 3.29E-03 0 0 -1.59E+00
GWP-fossil kg CO 2 eq 2.87E+00 7.47E-03 8.85E-03 0 3.28E-03 0 0 -1.59E+00
GWP-biogenic kg CO 2 eq -2.06E-01 3.74E-06 2.07E-01 0 1.64E-06 0 0 8.98E-05
GWP-luluc kg CO 2 eq 8.83E-04 2.88E-05 8.22E-07 0 1.26E-05 0 0 -4.7E-05
ODP kg CFC11 eq 3.16E-12 1.53E-15 3.46E-14 0 6.72E-16 0 0 -9.67E-13
AP mol H+ eq 6.99E-03 7.25E-06 4.65E-05 0 3.18E-06 0 0 -3.31E-03
EP-freshwater kg P eq 2.27E-06 1.49E-08 7.9E-09 0 6.54E-09 0 0 -4.69E-07
EP-marine kg N eq 1.62E-03 2.45E-06 1.32E-05 0 1.07E-06 0 0 -5.99E-04
EP-terrestrial mol N eq 1.75E-02 2.89E-05 2.22E-04 0 1.27E-05 0 0 -5.32E-03
kg NMVOC
POCP 5.27E-03 6.49E-06 3.46E-05 0 2.85E-06 0 0 -2.38E-03
eq
ADPE kg Sb eq 5.34E-06 7.49E-10 8.46E-10 0 3.29E-10 0 0 -3.76E-06
ADPF MJ 2.86E+01 9.92E-02 5.88E-02 0 4.35E-02 0 0 -1.51E+01
m3 world eq
WDP 1.83E-01 3.21E-05 2.62E-02 0 1.41E-05 0 0 -2.8E-01
deprived
GWP = Global warming potential; ODP = Depletion potential of the stratospheric ozone layer; AP = Acidification potential of land and water; EP =
Eutrophication potential; POCP = Formation potential of tropospheric ozone photochemical oxidants; ADPE = Abiotic depletion potential for non-fossil
resources; ADPF = Abiotic depletion potential for fossil resources; WDP = Water (user) deprivation potential)
RESULTS OF THE LCA - INDICATORS TO DESCRIBE RESOURCE USE according to EN 15804+A2: 1 kilogram Steel radiator
Parameter Unit A1-A3 A4 A5 C1 C2 C3 C4 D
PERE MJ 2.27E+00 6.53E-03 2.08E+00 0 2.86E-03 0 0 4.2E-01
PERM MJ 2.06E+00 0 -2.06E+00 0 0 0 0 0
PERT MJ 4.33E+00 6.53E-03 1.64E-02 0 2.86E-03 0 0 4.2E-01
PENRE MJ 2.87E+01 9.93E-02 1.44E-01 0 4.35E-02 0 0 -1.51E+01
PENRM MJ 8.55E-02 0 -8.55E-02 0 0 0 0 0
PENRT MJ 2.87E+01 9.93E-02 5.88E-02 0 4.35E-02 0 0 -1.51E+01
SM kg 1.89E-01 0 0 0 0 0 0 8.66E-01
RSF MJ 0 0 0 0 0 0 0 0
NRSF MJ 0 0 0 0 0 0 0 0
FW m3 4.3E-03 5.06E-06 6.16E-04 0 2.22E-06 0 0 -6.48E-03
PERE = Use of renewable primary energy excluding renewable primary energy resources used as raw materials; PERM = Use of renewable primary
energy resources used as raw materials; PERT = Total use of renewable primary energy resources; PENRE = Use of non-renewable primary energy
excluding non-renewable primary energy resources used as raw materials; PENRM = Use of non-renewable primary energy resources used as raw
materials; PENRT = Total use of non-renewable primary energy resources; SM = Use of secondary material; RSF = Use of renewable secondary fuels;
NRSF = Use of non-renewable secondary fuels; FW = Use of net fresh water
RESULTS OF THE LCA – WASTE CATEGORIES AND OUTPUT FLOWS according to EN 15804+A2:
1 kilogram Steel radiator
Parameter Unit A1-A3 A4 A5 C1 C2 C3 C4 D
HWD kg 2.51E-09 4.33E-13 6.27E-12 0 1.9E-13 0 0 -3.36E-10
NHWD kg 3.58E-02 1.62E-05 2.34E-03 0 7.08E-06 0 0 2.08E-01
RWD kg 5.74E-04 1.25E-07 1.91E-06 0 5.47E-08 0 0 -4.78E-05
CRU kg 0 0 0 0 0 0 0 0
MFR kg 5.51E-02 0 0 0 0 1E+00 0 0
MER kg 0 0 0 0 0 0 0 0
EEE MJ 0 0 3.14E-01 0 0 0 0 0
EET MJ 0 0 7.25E-01 0 0 0 0 0
4 Environmental Product Declaration - Kermi GmbH - Steel radiator
HWD = Hazardous waste disposed; NHWD = Non-hazardous waste disposed; RWD = Radioactive waste disposed; CRU = Components for re-use;
MFR = Materials for recycling; MER = Materials for energy recovery; EEE = Exported electrical energy; EET = Exported thermal energy
RESULTS OF THE LCA – additional impact categories according to EN 15804+A2-optional:
1 kilogram Steel radiator
Parameter Unit A1-A3 A4 A5 C1 C2 C3 C4 D
Disease
PM 1.15E-07 4.61E-11 2.49E-10 0 2.02E-11 0 0 -4.62E-08
incidence
IR kBq U235 eq 4.94E-02 1.27E-05 2.01E-04 0 5.56E-06 0 0 2.88E-02
ETP-fw CTUe 6.58E+00 7.59E-02 2.47E-02 0 3.33E-02 0 0 -1.07E+00
HTP-c CTUh 3.07E-09 1.52E-12 1.69E-12 0 6.68E-13 0 0 -6.27E-10
HTP-nc CTUh 3.16E-08 7.65E-11 6.61E-11 0 3.36E-11 0 0 -2.09E-08
SQP SQP 3.3E+01 2.97E-02 1.83E-02 0 1.3E-02 0 0 -1.38E-01
PM = Potential incidence of disease due to PM emissions; IR = Potential Human exposure efficiency relative to U235; ETP-fw = Potential comparative
Toxic Unit for ecosystems; HTP-c = Potential comparative Toxic Unit for humans (cancerogenic); HTP-nc = Potential comparative Toxic Unit for humans
(not cancerogenic); SQP = Potential soil quality index
Disclaimer 1 – for the indicator “Potential Human exposure efficiency relative to U235”. This impact category deals mainly with the
eventual impact of low-dose ionizing radiation on human health of the nuclear fuel cycle. It does not consider effects due to possible
nuclear accidents, occupational exposure or radioactive waste disposal in underground facilities. Potential ionizing radiation from the
soil, radon and from some construction materials is also not measured by this indicator.
Disclaimer 2 – for the indicators “abiotic depletion potential for non-fossil resources”, “abiotic depletion potential for fossil resources”,
“water (user) deprivation potential, deprivation-weighted water consumption”, “potential comparative toxic unit for ecosystems”,
“potential comparative toxic unit for humans – cancerogenic”, “Potential comparative toxic unit for humans - not cancerogenic”,
“potential soil quality index”. The results of this environmental impact indicator shall be used with care as the uncertainties on these
results are high as there is limited experience with the indicator.
References
Standards RAL-GZ 618
RAL-GZ 618:2017-08, Steel radiators - Qualitiy assessment
EN 442-1
DIN EN 442-1:2014, Radiators and convectors - Part 1: Further References
Technical specifications and requirements
BNB
EN 442-2 BBSR table (german): 'Nutzungsdauern von Bauteilen zur
DIN EN 442-2:2014, Radiators and convectors - Part 2: Test Lebenszyklusanalyse nach BNB', Bundesinstitut für Bau-,
methods and rating Stadt- und Raumforschung, Referat II Nachhaltiges Bauen;
online available under
ISO 14025 https://www.nachhaltigesbauen.de/austausch/nutzungsdauern-
DIN EN ISO 14025:2011-10: Environmental labels and von-bauteilen/
declarations — Type III environmental declarations —
Principles and procedures GaBi
Sphera Solutions GmbH GaBi Software System and Database
ISO 14040 for Life Cycle Engineering CUP Version: 2022.2 University of
EN ISO 14040:2006, Environmental management - Life cycle Stuttgart Leinfelden Echterdingen
assessment - Principles and framework.
GaBi documentation
ISO 14044 GaBi life cycle inventory data documentation
EN ISO 14044:2006, Environmental management - Life cycle (https://www.gabisoftware.com/support/gabi/gabidatab
assessment - Requirements and guidelines ase2020lcidocumentation/)
DIN EN 15804 IBU PCR PART A
EN 15804:2012+A2:2019+AC:2021, Sustainability of Product category rules for building- related products and
constructionworks — Environmental Product Declarations — services. Part A, PCR - Part A: Calculation Rules for the Life
Core rules for the product category of construction products Cycle Assessment and Requirements on the Project Report
according to EN 15804+A2:2019, version 1.3, Institut Bauen
EU No 305/2011 (CPR) und Umwelt e.V., www.ibu-epd.com, 2022
REGULATION (EU) No 305/2011 OF THE EUROPEAN
PARLIAMENT AND OF THE COUNCIL of 9 March 2011 laying IBU PCR Part B
down harmonised conditions for the marketing of construction PCR – Part B: Requirements on the EPD for Radiators, version
products and repealing Council Directive 89/106/EEC 1.0, Institut Bauen und Umwelt e.V., www.ibu-epd.com, 2023
EWC IBU 2021
European Waste Catalogue Institut Bauen und Umwelt e.V.: General Instructions for the
EPD programme of Institut Bauen und Umwelt e.V., Version
2.0, Berlin: Institut Bauen und Umwelt e.V., 2021
5 Environmental Product Declaration - Kermi GmbH - Steel radiator
Publisher
Institut Bauen und Umwelt e.V. +49 (0)30 3087748- 0
Hegelplatz 1 info@ibu-epd.com
10117 Berlin www.ibu-epd.com
Germany
Programme holder
Institut Bauen und Umwelt e.V. +49 (0)30 3087748- 0
Hegelplatz 1 info@ibu-epd.com
10117 Berlin www.ibu-epd.com
Germany
Author of the Life Cycle Assessment
Sphera Solutions GmbH +49 711 341817-0
Hauptstraße 111- 113 info@sphera.com
70771 Leinfelden-Echterdingen www.sphera.com
Germany
Owner of the Declaration
Kermi GmbH +49 (0) 9931 501-0
Pankofen-Bahnhof 1 info@kermi.de
94447 Plattling www.kermi.de
Germany
6 Environmental Product Declaration - Kermi GmbH - Steel radiator
