ENVIRONMENTAL PRODUCT DECLARATION
as per ISO 14025 and EN 15804+A2
Owner of the Declaration IGI - The Global Wallcoverings Association
Publisher Institut Bauen und Umwelt e.V. (IBU)
Programme holder Institut Bauen und Umwelt e.V. (IBU)
Declaration number EPD-IGI-20230436-IBG1-EN
Issue date 18.01.2024
Valid to 17.01.2029
Vinyl wallcoverings on woven textile backing
IGI - The Global Wallcoverings Association
www.ibu-epd.com | https://epd-online.com
1. General Information
IGI - The Global Wallcoverings Association Vinyl wallcoverings on woven textile backing
Programme holder Owner of the declaration
IBU – Institut Bauen und Umwelt e.V. IGI - The Global Wallcoverings Association
Hegelplatz 1 Chaussée de Louvain 426
10117 Berlin 1380 LASNE
Germany Belgium
Declaration number Declared product / declared unit
EPD-IGI-20230436-IBG1-EN The declared unit is 1m² (square meter) decorative vinyl based
wallcovering on woven textile backing including packaging.
This declaration is based on the product category rules: Scope:
Wall coverings, 01.08.2021 This EPD focuses on the production, transport and disposal of a weighted
(PCR checked and approved by the SVR) average of 1m² vinyl wallcoverings on woven textile backing of
participating members of the IGI - The Global Wallcoverings Association.
9 out of 71 IGI-members are involved in this EPD: A.S. Création Tapeten
Issue date AG (DE), Anstey Wallpaper Co. Ltd (GB), BN International (NL), J.
Josephson Inc. (US), JV S.p.A. (IT), Muraspec Decorative Solutions Ltd.
18.01.2024
(GB), Roysons Corporation (US), Versa Wallcovering (US), York
Wallcoverings Inc. (US).
The technical properties are displayed in chapter 2.3.
Valid to
The owner of the declaration shall be liable for the underlying information
17.01.2029 and evidence; the IBU shall not be liable with respect to manufacturer
information, life cycle assessment data and evidences.
The EPD was created according to the specifications of EN 15804+A2. In
the following, the standard will be simplified as EN 15804.
Verification
The standard EN 15804 serves as the core PCR
Independent verification of the declaration and data according to ISO
14025:2011
internally X externally
Dipl.-Ing. Hans Peters
(Chairman of Institut Bauen und Umwelt e.V.)
Florian Pronold Prof. Dr. Birgit Grahl,
(Managing Director Institut Bauen und Umwelt e.V.) (Independent verifier)
1 Environmental Product Declaration - IGI - The Global Wallcoverings Association - Vinyl wallcoverings on woven textile backing
2. Product
1a: Product according to the CPR, based on (BS) EN
2.1 Product description/Product definition 15102:
Vinyl wallcoverings on woven textile backing according to EN Performance data of the product in accordance with the
15102 involve plasticized PVC (vinyl) and a woven textile base. Declaration of Performance with respect to its Essential
The textile base (scrim) can be cotton or a polyester-cotton Characteristics according to EN 15102
blend. When the wallcovering is to be changed it can be
stripped in its entirety by peeling the wallcovering lengths from or:
the wall. This property as defined in EN 235 is strippable.
For the placing on the market of the product in the European 1b
Union/European Free Trade Association (EU/EFTA) (with the Performance Category I, II, III, IV, V or VI as described in Table
exception of Switzerland) Regulation (EU) No. 305/2011 (CPR) 1 of F 793-0-06 should be declared.
applies. The product needs a Declaration of Performance Or:
taking into consideration EN 15102 and CE-marking. Compliance with Wallcoverings Association WA-101 Type I, II
or III should be declared.
For the application and use the respective national provisions
apply. 2.4 Delivery status
The products declared are provided within the following
For the placing on the market in Great Britain the product dimensions:
needs a Declaration of Performance taking into consideration
(BS) EN 15102 and UK Conformity Assessed (UKCA) marking.
For placing on the market in Northern Ireland the product needs
a Declaration of Performance taking into consideration (BS) EN
15102 and CE or CE and UK Northern Ireland (UKNI) marking.
This table contains the range of all wallcoverings examined. For
For the placing on the market in the USA the product should more precise information please contact the specific
conform to ASTM F 1141 – 93 Standard Specification for manufacturer.
Wallcovering and ASTM F 793 – 06 Standard Classification of
2.5 Base materials/Ancillary materials
Wall Covering by Use Characteristics.
The weighted average of the primary product components is
Or: Wallcoverings Association WA-101 Quality Standard for shown in the following table, in percentage:
Polymer coated Fabric Wallcovering. Name Value Unit
Carrier material (Cotton) 8 %
2.2 Application
Packaging 15 %
Wallcoverings are used for the decorative wall design of interior
spaces in private or commercial use. Additives 13 %
PVC plastisol 62 %
2.3 Technical Data
Ink & Pigment 1 %
Name Value Unit
Sum 100 %
category 1 -
Measures by categories EN 233 - Pallets were considered as part of the packaging.
3
Straightness and parallelism according to
< 1 - This product contains substances listed in the candidate list
DIN EN 12956
(date: 06.12.2023) exceeding 0.1 percentage by mass: yes,
Washability according to EN 12956 extra- - C14-C17 chlorinated paraffin (containing < 1 % C10-13)
scrubbable (chlorination: 40 - 63 %) CAS no.: 85535-85-9.
Colour fastness to light according to EN ISO This product contains other CMR substances in categories 1A
6 -
105-B02 or 1B that are not on the candidate list, exceeding 0.1
Migration of heavy metals and certain other fulfills the percentage by mass: yes, vinyl acetate CAS no.: 108-05-4.
-
elements to EN 12149 norm Biocide products were added to this construction product or it
has been treated with biocide products (this then concerns a
Vinyl chloride monomer (VCM) content max. fulfills the
- treated product as defined by the (EU) Ordinance on Biocide
< 0,2 mg/m² according to EN 12149 norm
Products No. 528/2012): no.
Emissions of formaldehyde max. < 120 fulfills the
- Ancillary materials of the phthalate chemical group, specifically
mg/kg according to EN 12149 norm
Diisononyl phthalate (DINP) and Dioctyl Terephthalate (DOTP),
In case of multiple answers, values need to be examined remain on the product and serve the function of softeners.
depending on the manufacturer. Plasticizers can also be found in the products, in the plastisol
For USA manufactured products should be in accordance with used for vinyl finishing.
ASTM F 793-0-06 Table 1 Classification Criteria. This EPD is a weighted average of a Manufacturer Group
Or: regarding several producers and product references. Therefore,
Wallcoverings Association WA-101 Table 1 Physical Test it cannot be ruled out that individual wallcoverings may contain
Requirements. small amounts (>0.1% of product weight) of substances that
Depending on whether products are intended for the European, are included in the Substance of Very High Concern SVHC
UK or US market, the following performance data must be candidate list, the CMR substances in categories 1A or 1B list
declared. or ancillary materials and additives serving the function of fire
retardants, softeners or biocides.
This can be attributed, for example, to the contents of treated
2 Environmental Product Declaration - IGI - The Global Wallcoverings Association - Vinyl wallcoverings on woven textile backing
cotton fibers.
Further information can be obtained from the respective 2.12 Reference service life
manufacturer. Given the wallcovering is professionally installed, the reference
service life is 15 years according to experience values.
2.6 Manufacture Description of the influences on the ageing of the product when
The manufacturing process can be described with the help of applied in accordance with the rules of technology.
the following graphic:
2.13 Extraordinary effects
Fire
The reaction to fire performance according to EN 13501 is
shown in the following table:*
Fire protection
Name Value
Building material class B-D
Burning droplets s1-s3
Smoke gas development d0-d2
*This table contains the range of all wallcoverings examined.
For more precise information please contact the specific
manufacturer.
For USA information on fire performance according to ASTM E
84 Test method for Surface Burning Characteristics of Building
The order of manufacture may change and can slightly deviate
Materials.
for different producers.
2.7 Environment and health during manufacturing
Water
Compliance with statutory health and safety for personnel is
Product is not water resistant. There is no risk of a hazardous
ensured. Further, the energy and environmental management
environmental impact in the event of water flooding.
is certified for some members according to ISO 14001 and ISO
50001.
Mechanical destruction
For greater detail please contact the specific Manufacturer.
There is no risk of a hazardous environmental impact following
2.8 Product processing/Installation unforeseen mechanical destruction.
Depending on the manufacturers suggestion, the adhesive is
2.14 Re-use phase
applied to the back of the wallcovering or the substrate using a
The product is not re-usable.
wallpaper brush or short-napped roller. The wallcovering is
pressed against the wall and is cut along the top and bottom
2.15 Disposal
edges to fit the wall.
Wallcoverings are subject to the waste code 170904 (mixed
2.9 Packaging construction and demolition waste other than those mentioned
in 170901, 170902 and 170903) in accordance with the
The product is wrapped in clear schrink-wrap film, packed in
European Waste Catalogue (EWC).
corrugated cardboard boxes and palletised.
Wallcoverings can therefore be disposed of as normal
2.10 Condition of use household waste, that is in the dustbin or in additional refuse
There are no special features to be noted within the limits of sacks. Used wallcoverings should not be placed in the waste
normal and customary usage. paper bank. Most household waste is incinerated or landfilled
depending on regional legal regulations in the EU or in the US.
2.11 Environment and health during use
2.16 Further information
No environmental problems can be expected when the product
is handled and used properly. For further information please visit www.igiwallcoverings.org.
3. LCA: Calculation rules
most likely scenario by production volumes and the selected
3.1 Declared Unit datasets correspond to all regarded regions.
The declared unit is 1 m² of wallcovering including packaging.
The model is based on a weighted average of the produced 3.2 System boundary
square meters of each participating manufacturer. Type of the EPD: cradle to gate - with option.
The EPD is considered a declaration of an average product as
Declared unit
calculated from the output of several manufacturers (2b).
Name Value Unit
Declared unit 1 m2 Modules A1-3, A4 and A5
Grammage 0.512 kg/m2 The product stage begins with the consideration of the
production of the necessary raw materials and energies
Conversion factor to 1 kg 1.953 -
including all corresponding upstream processes as well as
Layer thickness 0.001 m
transport. Furthermore, the entire production phase was
Density 5128 kg/m3 investigated, including the treatment of production waste until
reaching the end-of-waste status (EoW). In addition, distribution
The production processes and location may vary between
transport and installation in the building were taken into
individual companies. The weighted average represents the
account.
3 Environmental Product Declaration - IGI - The Global Wallcoverings Association - Vinyl wallcoverings on woven textile backing
the basis of evaluations of the internal production and
Modules C1-4 environmental data, the collection of LCA-relevant data within
The modules include the removal and environmental impacts of the supply chain as well as through the measurement of
the waste treatment until reaching the end-of-waste status relevant energy supply data. The collected data were checked
(EoW) including the associated transport at the end of the for plausibility and consistency. A good representation is to be
product life cycle. assumed.
The data were collected in 2022 and refer to the calendar year
Module D 2021.
Calculation of potential benefits through the generated energy
(electric & thermic) by the incineration processes in the life 3.7 Period under review
cycle stages in A5 C3 and C4. The burdens resulting from the The LCA data were collected for the calendar year 2021.
waste-to-energy plants are assigned in module C3 or C4 in
3.8 Geographic Representativeness
case of landfill gas combustion.
Land or region, in which the declared product system is
3.3 Estimates and assumptions manufactured, used or handled at the end of the product´s
Most solvents were modelled as a generic mix of solvents. lifespan: Global
3.4 Cut-off criteria
3.9 Allocation
No materials were cut-off from the study. No energy
consumption was neglected. Potential benefits resulting from the thermal utilization of the
packaging waste (module A5) as well as from the thermal
3.5 Background data utilization or landfilling of the wallcoverings at the end of life
For modelling the lifecycle, the LCA for Experts Software (modules C3 and C4) are allocated to module D.
System and Database for Life Cycle Engineering (GaBi)
3.10 Comparability
Service pack 2023.1 was used. All background data records
relevant for production and disposal were almost exclusively Basically, a comparison or an evaluation of EPD data is only
taken from various GaBi supplementary databases or rarely possible if all the data sets to be compared were created
also from ecoinvent (v.3.6). The data records included in the according to EN 15804 and the building context, respectively
databases are documented online. the product-specific characteristics of performance, are taken
into account. The used background database is GaBi service
3.6 Data quality package 1 of 2023.
Data collection for the investigated products was carried out on
4. LCA: Scenarios and additional technical information
Installation into the building (A5)
Characteristic product properties of biogenic carbon
The treatment of packaging as waste was modeled in Module
The biogenic carbon content quantifies the amount of biogenic
A5 as a weighted average. The following table depicts the
carbon in a construction product leaving the factory gate, and it
packaging materials treated in A5 with more than 1 gram of
is separately declared for the product and for any
participation in the weighted average.
accompanying packaging.
Modules B1-B7 are deemed not relevant since the product
Information on describing the biogenic Carbon Content at needs no maintenance or operational energy or water use and
factory gate are, therefore, not declared.
Name Value Unit Name Value Unit
Biogenic carbon content in product 0.0001 kg Polyethylene 0.065 kg
C
Cardboard 0.007 kg
Biogenic carbon content in accompanying kg
0.0028 Pallet 0.004 kg
packaging C
Note: 1 kg of biogenic carbon is equivalent to 44/12 kg of CO . Reference service life
2
Name Value Unit
Reference service life 15 a
End of life (C1-C4)
Transport to the building site (A4)
Name Value Unit
Name Value Unit
Energy recovery 4 %
Truck transport 27 t payload
Landfilling 96 %
Transport distance 2462 km
Train transport 726 t payload For the calculation of this LCA landfilling is chosen for the US
and incineration for the EU. Different disposal routes are
Transport distance 3 km
available but not taken into account for this industry average
Ship transport 27500 dwt payload
LCA.
Transport distance 912 km
Cargo plane transport 65 t payload Reuse, recovery and/or recycling potentials (D), relevant
Transport distance 41 km scenario information
In module D the potential benefits of the thermal combustion
Capacity utilisation (including empty runs) 80 - 90 %
from the wallcoverings (C3), their packaging (A5) as well as the
Because many different countries are involved, there were incineration of landfill gases (C4) are displayed.
always global data sets used to model the transport distances.
4 Environmental Product Declaration - IGI - The Global Wallcoverings Association - Vinyl wallcoverings on woven textile backing
5. LCA: Results
In this section, the LCA results for 1 m² wallcoverings are presented. It should be borne in mind that the LCA results only indicate
possible effects.
Indicators used for evaluation:
The EN 15804+A2 LCIA methodology with the characterization factors infrom EU-JRC were used to evaluate the possible
environmental effects of the wallcoverings. The characterization factors are available at the following internet link:
http://eplca.jrc.ec.europa.eu/LCDN/developerEF.xhtml.
DESCRIPTION OF THE SYSTEM BOUNDARY (X = INCLUDED IN LCA; MND = MODULE OR INDICATOR NOT DECLARED; MNR
= MODULE NOT RELEVANT)
Benefits and
Construction loads beyond
Product stage Use stage End of life stage
process stage the system
boundaries
la ire ta m w a Ry lp p u s tro p s n a rT g n iru tc a fu n a M e h t m o rf tro p s n a rTe tis e h t o t e ta g y lb m e s s A e s U e c n a n e tn ia M ria p e R tn e m e c a lp e R tn e m h s ib ru fe R y g re n e la n o ita re p Oe s u re ta w la n o ita re p Oe s u n o itc u rts n o c -e Dn o itilo m e d tro p s n a rT g n is s e c o rp e ts a W la s o p s iD -e s u e R-y re v o c e R-g n ilc y c e Rla itn e to p
A1 A2 A3 A4 A5 B1 B2 B3 B4 B5 B6 B7 C1 C2 C3 C4 D
X X X X X MND MND MNR MNR MNR MND MND X X X X X
RESULTS OF THE LCA - ENVIRONMENTAL IMPACT according to EN 15804+A2: 1 m² vinyl wallcoverings on woven textile
backing
Parameter Unit A1-A3 A4 A5 C1 C2 C3 C4 D
GWP-total kg CO 2 eq 1.51E+00 2.01E-01 1.63E-02 2.66E-05 4.11E-03 2.75E-02 3.02E-02 -1.15E-02
GWP-fossil kg CO 2 eq 1.52E+00 2E-01 5.89E-03 2.66E-05 4.07E-03 2.71E-02 3.02E-02 -1.15E-02
GWP-biogenic kg CO 2 eq -1.08E-02 0 1.04E-02 0 0 3.53E-04 0 0
GWP-luluc kg CO 2 eq 3.35E-04 1.03E-03 1.02E-05 8.9E-09 3.75E-05 1.39E-06 2.32E-05 -7.95E-07
ODP kg CFC11 eq 4.92E-09 1.95E-14 8.55E-15 1.62E-16 5.27E-16 1.42E-14 4.45E-14 -1.02E-13
AP mol H+ eq 4.46E-03 1.31E-03 2.17E-05 6.74E-08 3.39E-05 1.03E-05 8.76E-05 -1.53E-05
EP-freshwater kg P eq 1.08E-05 4.22E-07 9.07E-07 2.34E-09 1.48E-08 4.48E-09 5.4E-06 -2.1E-08
EP-marine kg N eq 1.06E-03 5.88E-04 7.38E-06 2.36E-08 1.69E-05 3.81E-06 3.34E-05 -4.34E-06
EP-terrestrial mol N eq 1.14E-02 6.48E-03 7.51E-05 1.63E-07 1.86E-04 4.76E-05 2.36E-04 -4.63E-05
kg NMVOC
POCP 3.6E-03 1.31E-03 2.03E-05 4.42E-08 3.19E-05 1.02E-05 8.11E-05 -1.2E-05
eq
ADPE kg Sb eq 3.78E-07 8.21E-09 1.75E-10 1.53E-12 2.67E-10 1.23E-10 7.41E-10 -9.2E-10
ADPF MJ 3.32E+01 2.69E+00 8.26E-02 4.75E-04 5.51E-02 3.08E-02 4.01E-01 -2.14E-01
m3 world eq
WDP 9.79E-01 1.47E-03 2.63E-04 8.61E-03 4.89E-05 3.23E-03 -1.28E-04 -1.24E-03
deprived
GWP = Global warming potential; ODP = Depletion potential of the stratospheric ozone layer; AP = Acidification potential of land and water; EP =
Eutrophication potential; POCP = Formation potential of tropospheric ozone photochemical oxidants; ADPE = Abiotic depletion potential for non-fossil
resources; ADPF = Abiotic depletion potential for fossil resources; WDP = Water (user) deprivation potential)
RESULTS OF THE LCA - INDICATORS TO DESCRIBE RESOURCE USE according to EN 15804+A2: 1 m² vinyl wallcoverings on
woven textile backing
Parameter Unit A1-A3 A4 A5 C1 C2 C3 C4 D
PERE MJ 2.61E+00 1.15E-01 1.79E-01 9.68E-05 4.01E-03 1.32E-02 3.64E-02 -6.98E-02
PERM MJ 1.78E-01 -1.72E-01 -5.65E-03 0 0 -5.65E-03 0 0
PERT MJ 2.79E+00 1.15E-01 7.4E-03 9.68E-05 4.01E-03 7.54E-03 3.64E-02 -6.98E-02
PENRE MJ 1.92E+01 2.7E+00 3.06E+00 4.76E-04 5.53E-02 3.5E-01 1.11E+01 -2.14E-01
PENRM MJ 1.4E+01 0 -2.98E+00 0 0 -3.19E-01 -1.07E+01 0
PENRT MJ 3.32E+01 2.7E+00 8.27E-02 4.76E-04 5.53E-02 3.09E-02 4.01E-01 -2.14E-01
SM kg 1.09E-04 0 0 0 0 0 0 0
RSF MJ 0 0 0 0 0 0 0 0
NRSF MJ 0 0 0 0 0 0 0 0
FW m3 2.42E-02 1.27E-04 9.06E-06 2E-04 4.39E-06 7.87E-05 9.96E-06 -5.65E-05
PERE = Use of renewable primary energy excluding renewable primary energy resources used as raw materials; PERM = Use of renewable primary
energy resources used as raw materials; PERT = Total use of renewable primary energy resources; PENRE = Use of non-renewable primary energy
excluding non-renewable primary energy resources used as raw materials; PENRM = Use of non-renewable primary energy resources used as raw
materials; PENRT = Total use of non-renewable primary energy resources; SM = Use of secondary material; RSF = Use of renewable secondary fuels;
NRSF = Use of non-renewable secondary fuels; FW = Use of net fresh water
RESULTS OF THE LCA – WASTE CATEGORIES AND OUTPUT FLOWS according to EN 15804+A2:
1 m² vinyl wallcoverings on woven textile backing
Parameter Unit A1-A3 A4 A5 C1 C2 C3 C4 D
HWD kg 1.45E-06 7.04E-12 6.18E-12 1.35E-14 1.71E-13 2.47E-13 3.39E-11 -8.09E-12
NHWD kg 6.32E-02 3.38E-04 6.9E-02 6.09E-05 8.44E-06 7.7E-03 4.09E-01 -1.11E-04
5 Environmental Product Declaration - IGI - The Global Wallcoverings Association - Vinyl wallcoverings on woven textile backing
RWD kg 9.04E-04 3.94E-06 9.17E-07 1.9E-08 1.04E-07 9.99E-07 4.74E-06 -1.85E-05
CRU kg 0 0 0 0 0 0 0 0
MFR kg 0 0 0 0 0 0 0 0
MER kg 1.6E-03 0 1.61E-03 0 0 1.63E-02 0 0
EEE MJ 4.68E-03 0 0 0 0 0 0 6.17E-02
EET MJ 8.08E-03 0 0 0 0 0 0 8.74E-02
HWD = Hazardous waste disposed; NHWD = Non-hazardous waste disposed; RWD = Radioactive waste disposed; CRU = Components for re-use;
MFR = Materials for recycling; MER = Materials for energy recovery; EEE = Exported electrical energy; EET = Exported thermal energy
RESULTS OF THE LCA – additional impact categories according to EN 15804+A2-optional:
1 m² vinyl wallcoverings on woven textile backing
Parameter Unit A1-A3 A4 A5 C1 C2 C3 C4 D
Disease
PM 9.74E-08 6.86E-09 1.94E-10 1.08E-12 2.41E-10 1.15E-10 8.6E-10 -1.3E-10
incidence
IR kBq U235 eq 5.57E-01 5.74E-04 1.36E-04 2.91E-06 1.54E-05 1.29E-04 6.98E-04 -3.08E-03
ETP-fw CTUe 1.1E+01 1.9E+00 7.59E-02 9.78E-04 3.92E-02 1.8E-02 4.1E-01 -5.23E-02
HTP-c CTUh 9.14E-10 3.72E-11 3.33E-12 1.86E-14 8.07E-13 9.37E-13 1.8E-11 -2.46E-12
HTP-nc CTUh 8.76E-08 2.08E-09 2.84E-10 1.74E-12 4.88E-11 8.68E-11 1.55E-09 -7.4E-11
SQP SQP 6.39E+00 6.38E-01 1.03E-02 7.07E-05 2.3E-02 7.08E-03 3.55E-02 -4.59E-02
PM = Potential incidence of disease due to PM emissions; IR = Potential Human exposure efficiency relative to U235; ETP-fw = Potential comparative
Toxic Unit for ecosystems; HTP-c = Potential comparative Toxic Unit for humans (cancerogenic); HTP-nc = Potential comparative Toxic Unit for humans
(not cancerogenic); SQP = Potential soil quality index
Disclaimer 1 – for the indicator “Potential Human exposure efficiency relative to U235”. This impact category deals mainly with the
eventual impact of low-dose ionizing radiation on human health of the nuclear fuel cycle. It does not consider effects due to possible
nuclear accidents, occupational exposure or radioactive waste disposal in underground facilities. Potential ionizing radiation from the
soil, radon and from some construction materials is also not measured by this indicator.
Disclaimer 2 – for the indicators “abiotic depletion potential for non-fossil resources”, “abiotic depletion potential for fossil resources”,
“water (user) deprivation potential, deprivation-weighted water consumption”, “potential comparative toxic unit for ecosystems”,
“potential comparative toxic unit for humans – cancerogenic”, “Potential comparative toxic unit for humans - not cancerogenic”,
“potential soil quality index”. The results of this environmental impact indicator shall be used with care as the uncertainties on these
results are high as there is limited experience with the indicator.
This EPD was created using a software tool.
6. LCA: Interpretation
6 Environmental Product Declaration - IGI - The Global Wallcoverings Association - Vinyl wallcoverings on woven textile backing
energy demands. Moreover, woven cotton fabric production has
The production stage (module A1-A3) clearly dominates the the largest influence on the acidification potential (AP), and the
LCA results. The loads caused by the disposal stage (modules eutrophication potential (EP). It is the second highest impact
C3 and C4) become noticeable, especially as the biogenic source, after PVC plastisol in the ozone depletion potential
carbon leaves the product system, reflected in the total and (ODP) and the potential for the formation of tropospheric ozone
biogenic global warming potential. Transports play a (POCP).
subordinate yet not insignificant role. Transport processes also affect GWP-fossil, AP, EP, POCP, and
The main environmental impacts are in all categories located in ADPF. The main reason is the combustion of fuels.
module A1-A3. For GWP-fossil and ADPF the highest precursor The waste treatment in module C3 in the GWP-fossil impact is
of impact is the use of PVC plastisol for vinyl coating. The dominated by the incineration of PVC plastisol at End-of-Life.
production of woven cotton fabric is the second-highest source
of GWP-fossil and ADPF. The production and use of thermal Range of the results
and electric energy for general production and heating/drying The individual results of the participating companies differ from
processes in A3 is the third highest precursor in both the average results in the present environmental product
categories. declaration. Regarding GWP, the results may be 92% higher or
The highest source of environmental impact in most categories 80% lower than the average for this EPD.
is the production of PVC plastisol, not only because it The main reason for the deviations is differences in the
constitutes 62% of the product mass; but because of the grammage of the individual wallcoverings. In addition, there are
energy-intensive production of PVC itself. different materials used as well as varying heat and electricity
The production of woven cotton fabric has a substantial effect. consumptions depending on the manufacturer.
It has a relatively high share of the greenhouse potential due to
7. Requisite evidence
Members of the The Global Wallcoverings Association have the wallcoverings meet the requirements of test standard
following certificates: ISO 16000.
• Optional compliance with German RAL-GZ 479.
• The declared products comply with EN 15102.
• Optional compliance with USA Wallcovering Association
• According to the (emission) test chamber assessment,
W-101 (2013) paragraph 8.1 when tested by California
which follows the French measurement method Arrêté
Specification Section 01350 to criteria CDPH/EHLB
du 19/04/11 the wallcoverings meet the requirements of
Standard Method V1.1 (2010).
the test standard ISO 16000.
The certificates and classifications for the various wallcoverings
• Optional according to the chamber test which follows
can be obtained from the respective manufacturers.
the German AgBB (Committee for health-related
evaluation of building products) regulations the
8. References
Standards and Norms
EN 12956:1999
Arrêté du 19/04/11 Wallcoverings in roll form - Determination of dimensions,
Order of 19 April 2011 relating to the labeling of construction straightness, spongeability and washability.
products or wall or floor coverings and paints and varnishes on
their emissions of volatile pollutants EN 13501-1:2018
Fire classification of construction products and building
ASTM E 84 elements - Part 1: Classification using data from reaction to fire
ASTM E 84:2016: Standard Test Method for Surface Burning Tests.
Characteristics of Building Materials
EN 15102:2007+A1:2011
ASTM F 793 Decorative wallcoverings - Roll and panel form.
ASTM F793 / F793M-15, Standard Classification of Wall
Coverings by Use Characteristics, ASTM International, West EN 233:2016
Conshohocken, PA, 2015 Wallcoverings in roll form - Specification for finished wallpapers,
wall vinyls and plastics wallcoverings.
ASTM F1141 - 93
ASTM F1141-93(2009), Standard Specification for EN 234:2019
Wallcovering, ASTM International, West Conshohocken, PA, Wallcoverings in roll form – Specification for wallcoverings for
2009 subsequent decoration
BNB EN 235:2001
Lifetimes of components for life cycle analyses according to the Wallcoverings - Vocabulary and Symbols.
Bewertungssystem Nachhaltiges Bauen, 2011.
EN 259-1:2001
CDPH/EHLB Wallcoverings in roll form - Heavy duty wallcoverings - Part 1:
Standard method for measuring and evaluating chemical Specifications.
emissions from indoor sources using environmental chambers,
Version 1.1 EN ISO 105-B02
Textiles - Tests for colour fastness - Part B02: Colour fastness
CPR to artificial light: Xenon arc fading lamp test (ISO 105-
Construction Product Regulation EU B02:2014).
7 Environmental Product Declaration - IGI - The Global Wallcoverings Association - Vinyl wallcoverings on woven textile backing
89/106/EEC Text with EEA relevance. Current consolidated
EN ISO 14025:2006 version: 16/07/2021
Environmental labels and declarations — Type III
environmental declarations — Principles and procedures; 2009- WA-101
11. WA Quality Standard for Polymer Coated Fabric Wallcovering
EN ISO 14044:2006
Environmental management - Life cycle assessment - Further documentation
Requirements and guidelines (ISO 14044:2006).
Ecoinvent
EN ISO 16000:2006 Database for Life Cycle Assessment, version 3.6. Swiss Center
Indoor air - Part 3: Determination of formaldehyde and other for Life Cycle Inventories, St. Gallen, 2023.
carbonyl compounds in indoor air and test chamber air - Active
sampling method. European Commission
Indoor air - Part 6: Determination of volatile organic compounds List of substances banned for use in cosmetic products. CMR
in indoor and test chamber air by active sampling on Tenax substances of category 1A, 1B or 2 under Commission
TA® sorbent, thermal desorption and gas chromatography Regulation (EC) No 790/2009. 01/12/2010. Updated
using MS or MS-FID. 01/07/2015.
Indoor air - Part 9: Determination of the emission of volatile
organic compounds from building products and furnishing - European Parliament
Emission test chamber method. Regulation (EU) no 528/2012 of the European Parliament and
Indoor air - Part 11: Determination of the emission of volatile of the council of 22 may 2012 concerning the making available
organic compounds from building products and furnishing - on the market and use of biocidal products.
Sampling, storage of samples and preparation of test
specimens. European Waste Catalogue (EWC)
European Waste Catalogue / Ordinance on European List of
ISO 14001:2015 Wastes
Environmental management systems - Requirements with
guidance for use. EU-JRC
EN 15804 reference package. Flows, Methods,
EN 15804 Characterisation Factors, Unit Groups and Flow Properties
EN 15804:2012+A2:2019+AC:2021, Sustainability of based on EF Reference Package 3.0.
construction works — Environmental Product Declarations —
Core rules for the product category of construction products. German AgBB
Committee for health-related evaluation of building products.
ISO 50001:2011 Umweltbundesamt Deutschlands.
Energy management systems - Requirements with guidance for
use. Institut Bauen und Umwelt e. V.
Product Category Rules for Building-Related Products and
SVHC Services – PCR-A: Part A+A2: Calculation Rules for the Life
Candidate List of substances of very high concern for Cycle Assessment and Requirements on the Project Report
Authorisation (SVHC) according to EN 15804+A2:2019, version: 1.3 from 31/08/2022.
Published in accordance with Article 59(10) of the REACH
Regulation. European chemicals agency (ECHA). Institut Bauen und Umwelt e. V.
PCR Guidance-Texts for Building-Related Products and
RAL-GZ 479 Services - Part B: Requirements on the EPD for Wallcoverings.
Wallpapers - Quality assurance Version: 8 from 01/08/2021.
Regulation (EU) No 305/2011 LCA for Experts (GaBi)
of the European Parliament and of the Council of 9 March 2011 LCA for Experts 10.7.0.183: Software System and Database for
laying down harmonised conditions for the marketing of Life Cycle Engineering. 1992-2023. Sphera Solutions GmbH
construction products and repealing Council Directive
8 Environmental Product Declaration - IGI - The Global Wallcoverings Association - Vinyl wallcoverings on woven textile backing
Publisher
Institut Bauen und Umwelt e.V. +49 (0)30 3087748- 0
Hegelplatz 1 info@ibu-epd.com
10117 Berlin www.ibu-epd.com
Germany
Programme holder
Institut Bauen und Umwelt e.V. +49 (0)30 3087748- 0
Hegelplatz 1 info@ibu-epd.com
10117 Berlin www.ibu-epd.com
Germany
Author of the Life Cycle Assessment
brands & values GmbH +49 421 70 90 84 33
Altenwall 14 info@brandsandvalues.com
28195 Bremen www.brandsandvalues.com
Germany
Owner of the Declaration
IGI - The Global Wallcoverings Association +32 (0) 2 720 00 09
Chaussée de Louvain 426 info@igiwallcoverings.org
1380 LASNE www.igiwallcoverings.org
Belgium
9 Environmental Product Declaration - IGI - The Global Wallcoverings Association - Vinyl wallcoverings on woven textile backing
