ENVIRONMENTAL PRODUCT DECLARATION
as per ISO 14025 and EN 15804+A2
Owner of the Declaration Olam Agri - Congolaise Industrielle des Bois
Publisher Institut Bauen und Umwelt e.V. (IBU)
Programme holder Institut Bauen und Umwelt e.V. (IBU)
Declaration number EPD-CON-20240291-CBA1-EN
Issue date 29.11.2024
Valid to 28.11.2029
Sapelli finger-jointed/laminated scantlings
Olam Agri
www.ibu-epd.com | https://epd-online.com
General Information
Olam Agri Sapelli finger-jointed/laminated scantlings
Programme holder Owner of the declaration
IBU – Institut Bauen und Umwelt e.V. Olam Agri - Congolaise Industrielle des Bois
Hegelplatz 1 Pokola BP 41
10117 Berlin BP 41 Ouesso
Germany (Others)
Declaration number Declared product / declared unit
EPD-CON-20240291-CBA1-EN Sapelli finger-jointed, solid or laminated scantlings, per cubic meter (m3)
This declaration is based on the product category rules: Scope:
Solid wood products, 01.08.2021
(PCR checked and approved by the SVR) This Environmental Product Declaration refers to Sapelli non-structural
scantlings that are produced out of wood that is harvested, sawn, air-dried,
kiln-dried, finger-jointed, and possibily laminated by the Congolaise
Issue date Industrielle des Bois (CIB).
CIB's forestry concessions and industrial site are located in the Republic of
29.11.2024
the Congo, Sangha department (site of Pokola) and Likouala department
(site of Enyelle).
CIB forests and production are 100% FSC certified.
Valid to
28.11.2029 This life cycle analysis is based on data from 2023.
CIB is fully owned by Olam Global Agri Pte. Ltd.
The owner of the declaration shall be liable for the underlying information
and evidence; the IBU shall not be liable with respect to manufacturer
information, life cycle assessment data and evidences.
The EPD was created according to the specifications of EN 15804+A2. In
the following, the standard will be simplified as EN 15804.
Verification
Dipl.-Ing. Hans Peters The standard EN 15804 serves as the core PCR
(Chairman of Institut Bauen und Umwelt e.V.)
Independent verification of the declaration and data according to ISO
14025:2011
internally X externally
Florian Pronold Angela Schindler,
(Managing Director Institut Bauen und Umwelt e.V.) (Independent verifier)
1 Environmental Product Declaration - Olam Agri - Sapelli finger-jointed/laminated scantlings
Product
Product description/Product definition For the use and application of the product the respective
Sapelli scantlings are fixed thickness, width and length wood national provisions at the place of use apply, in Germany for
scantlings. They can be composed of one or several lamellas example the building codes of the federal states and the
finger-jointed and glued together. corresponding national specifications.
Scantlings produced according to the following process: Application
Trees are inventoried, counted, and harvested as per our forest Sapelli scantlings (non-structural) are mostly used in doors and
management plans. windows frame manufacturing (exterior joinery) but can also be
used in interior joinery and furniture manufacturing.
Logs are exported to CIB facilities in Pokola and Enyelle, sorted
by quality and sawn in one of CIB's sawmills according to Technical Data
customer requirements for length, thickness, width, and quality. Technical data on Sapelli wood can be found on the CIRAD's
Lumber that does not fall within these requirements is Tropix database at the following link:
recovered and bundled. https://tropix.cirad.fr/FichiersComplementaires/EN/Africa/SAPELLI.pdf.
Constructional data
Lumber is stacked on stickers and left on our site for air-drying
Name Value Unit
for a period varying between 3 weeks to 6 months, depending
Wood types by trade names acc. to TROPIX Sapelli -
on the thickness.
Wood moisture 8 - 18 %
When the wood has reached its fiber saturation point, it is taken Gross density acc. to TROPIX 690 kg/m3
into our kilns for a drying cycle varying between 3 days to 6
Risk class acc. to TROPIX Class 3 -
weeks. Final moisture content depends on customer
requirements and usually varies from 8% to 16%. Performance data of the product with respect to its
characteristics in accordance with the relevant technical
After kilning, bundles are destacked, and planks are sorted by provision (no CE-marking).
widths (if it hasn't been done after sawing).
Base materials/Ancillary materials
The wood specie of this lumber is Sapelli (entandrophragma
Wood pieces undergo several steps of calibration in length,
cylindricum).
width, and thickness.
The glue used for finger-jointed and lamination is a two-
After a blanking operation (revealing defects), wood pieces are
components EPI glue and hardener.
sorted by quality type. Pieces are then finger-jointed end-to-end
This product contains substances listed in the candidate list
to create a solid finger-jointed scantling or a lamella for
(date: 17.10.2023) exceeding 0.1 percentage by mass: no
lamination.
This product contains other Carcinogenic, Mutagenic,
Solid finger-jointed scantlings are then molded, cut to final
Reprotoxic (CMR) substances in categories 1A or 1B which are
length, bundled, and marked for export.
not on the candidate list, exceeding 0.1 percentage by mass:
no
Lamellas are planed, glued, and pressed for a certain amount
of time, depending on the glue/hardener ratio and production
Biocide products were added to this construction product or it
conditions (humidity, temperature, moisture content of the
has been treated with biocide products (this then concerns a
wood, etc.). The press is unloaded, and after a curing period,
treated product as defined by the (EU) Ordinance on Biocide
the laminated scantlings are then molded, cut to final length,
Products No. 528/2012): no
bundled, and marked for export.
Reference service life
The glue used for finger-jointed and lamination is a two-
Depending on how and where it is used (internal, external) and
components EPI glue and hardener.
various conditions (weather, exposition to sun, rain, humidity),
Sapelli lumber is durable for several decades.
All along the production process, an internal quality control
team performs tests, samples, and analyzes the samples in a
Scantlings are a pre-product and will then be moulded and
laboratory to ensure that the production procedures are
protected.
respected and that the products meet the required quality.
LCA: Calculation rules
Name Value Unit
Declared Unit
Declared unit 1 m3
The declaration refers to the declared unit of 1m³ of Sapelli
finger-jointed/laminated scantling. The density of the final Gross density 690 kg/m3
product is 690kg/m³. Wood moisture (upon delivery) 12 %
Declared unit and mass reference Water content = 11%
Moisture content = 12%
System boundary
2 Environmental Product Declaration - Olam Agri - Sapelli finger-jointed/laminated scantlings
The type of EPD is cradle to gate with options, module C1-C4, energy, which result from energy recovery in modules
and module D (A1-A3, C, D and additionnal modules A4 and A5 and C3) are declared in module D.
A5). • The CO2 incorporation in the product (from the
sequestration in the wood) is considered. The C-balance
Considered product stages: is closed by considering the biotic GHG emissions
according to the incorporation on input side.
• Production of raw materials (e.g. log extraction from the
The data collected by the manufacturers is based on yearly
forest), extraction of energy carriers, raw material
production amounts. The production data refers to the yearly
transportation, manufacture of product and packaging
consumption in 2023.
materials are declared in modules A1-A3. Modules A1-
A3 also include the generation and supply of energy (on
Geographic Representativeness
site production via biomass power plant).
Land or region, in which the declared product system is
• The scenario for the transport of the product to the
manufactured, used or handled at the end of the product´s
construction site is declared in module A4.
lifespan: Global
• The treatment of packaging materials at installation is
declared in module A5. Sapelli finger-jointed/laminated
scantling is a pre- product, the installation of such Comparability
product is very variable. The installation stage (e.g.
Basically, a comparison or an evaluation of EPD data is only
installation process and potential auxiliaries) has been
possible if all the data sets to be compared were created
excluded from the scope of the study.
according to EN 15804 and the building context, respectively
• The end-of-life scenarios include, deconstruction (C1),
the product-specific characteristics of performance, are taken
transportation to waste processing (C2), emissions and
into account. Background dataset : GaBi ts software, CUP
energy requirements of combustion (C3). Benefits and
2022.1.
loads for the next system (e.g. electricity and thermal
LCA: Scenarios and additional technical information
Packaging materials:
Characteristic product properties of biogenic carbon Plastic film : 0,20 kg/m³
The product and packaging material (wooden wedges) contains Plastic straps : 0,84 kg/m³
biogenic carbon. The following biogenic carbon content is Steel straps : 0,11 kg/m³
assumed : Steel buckles: 0,11 kg/m³
- 0,484kg C /kg of hardwood wood (dry) Wooden wedges: 3,60 kg/m³
- 0,5kg C /kg of wooden wedges (dry)
Information on describing the biogenic carbon content at End of life (C1-C4)
factory gate The end-of-life scenarios are as follows:
Name ValueUnit
kg C1 – Dismantling / Demolition: Sapelli finger-jointed/laminated
Biogenic carbon content in product 298
C scantling is a pre-product and the deconstruction scenario is
unknown as it has multiple uses. The most common use for this
Biogenic carbon content in accompanying kg
1.48 product being doors and windows frames we have considered
packaging C
that the product could be manually dismounted and therefore
Note: 1 kg of biogenic carbon is equivalent to 44/12 kg of CO 2. the result for C1 is "0".
C2 – Transport to treatment/disposal site: Average transport
The following technical scenario information is required for the distance from the demolition site to waste treatment is assumed
declared modules. as 50 km to thermal treatment.
Transport to the building site (A4)
C3 – Waste treatment: Sapelli finger-jointed/laminated scantling
The transportation of the Sapelli scantlings from the
is 100 % combusted with energy recovery.
manufacturing plant in Pokola, Republic of Congo to the
construction site in Europe is considered.
C4 – Disposal: No disposal scenario.
Name Value Unit
Name Value Unit
Litres of fuel 1.52 l/100km
Energy recovery 690 kg
Transport distance 1250 km
Capacity utilisation (including empty runs) 61 % Reuse, recovery and/or recycling potentials (D), relevant
Gross density of products transported 690 kg/m3 scenario information
Name Value Unit
Transport distance (ocean ship) 8426 kms
For the thermal and electrical energy generated in module A5
Installation into the building (A5)
due to thermal treatment of packaging and C3 for the
Module A5 includes the waste processing up to the end-of- incineration of the product, avoided burdens have been
waste state or disposal of packaging materials during the calculated by the inversion of electricity grid mix and thermal
construction process stage. The installation stage (e.g. energy from natural gas, using European datasets. Material
installation process and potential auxiliaries) has been benefits are also given for the recycling of metal packaging
excluded from the scope of the study. materials (steel buckles and steel straps).
Name ValueUnit
Output substances following waste treatment on
4.86 kg
site
3 Environmental Product Declaration - Olam Agri - Sapelli finger-jointed/laminated scantlings
LCA: Results
The following tables display the environmentally relevant results according to EN 15804+A2 (EF 3.0) for 1 m³ of Sapelli finger-
jointed/laminated scantlings.
Please be aware, the module A5 only considers the disposal of packaging material, and do not the complete installation scenario
because the declared product is a pre-product and installation is unknown.
DESCRIPTION OF THE SYSTEM BOUNDARY (X = INCLUDED IN LCA; MND = MODULE OR INDICATOR NOT DECLARED; MNR
= MODULE NOT RELEVANT)
Benefits and
Construction loads beyond
Product stage Use stage End of life stage
process stage the system
boundaries
la ire ta m w a Ry lp p u s tro p s n a rT g n iru tc a fu n a M e h t m o rf tro p s n a rTe tis e h t o t e ta g y lb m e s s A e s U e c n a n e tn ia M ria p e R tn e m e c a lp e R tn e m h s ib ru fe R y g re n e la n o ita re p Oe s u re ta w la n o ita re p Oe s u n o itc u rts n o c -e Dn o itilo m e d tro p s n a rT g n is s e c o rp e ts a W la s o p s iD -e s u e R-y re v o c e R-g n ilc y c e Rla itn e to p
A1 A2 A3 A4 A5 B1 B2 B3 B4 B5 B6 B7 C1 C2 C3 C4 D
X X X X X MND MND MNR MNR MNR MND MND X X X X X
RESULTS OF THE LCA - ENVIRONMENTAL IMPACT according to EN 15804+A2: 1 m3 Sapelli finger-jointed/laminated
scantling
Parameter Unit A1-A3 A4 A5 C1 C2 C3 C4 D
GWP-total kg CO 2 eq -8.93E+02 1.09E+02 8.1E+00 0 2.42E+00 1.1E+03 0 -3.63E+02
GWP-fossil kg CO 2 eq 2.02E+02 1.06E+02 2.7E+00 0 2.3E+00 1.88E+01 0 -3.61E+02
GWP-biogenic kg CO 2 eq -1.1E+03 2.54E+00 5.4E+00 0 1.08E-01 1.08E+03 0 -1.85E+00
GWP-luluc kg CO 2 eq 8.04E-01 6.21E-04 4.14E-05 0 1.55E-02 2.71E-03 0 -3.97E-02
ODP kg CFC11 eq 7.52E-11 3.9E-13 8.73E-13 0 2.26E-13 1.25E-10 0 -2.44E-09
AP mol H+ eq 9.32E+00 1.87E+00 1.11E-03 0 2.58E-03 1.64E-01 0 -4.76E-01
EP-freshwater kg P eq 4.4E-03 2.02E-05 2.19E-07 0 8.23E-06 2.82E-05 0 -4.97E-04
EP-marine kg N eq 2.81E+00 4.91E-01 3.46E-04 0 8.34E-04 5.3E-02 0 -1.29E-01
EP-terrestrial mol N eq 4.33E+01 5.38E+00 5.22E-03 0 9.98E-03 7.65E-01 0 -1.38E+00
kg NMVOC
POCP 3.1E+01 1.38E+00 9.54E-04 0 2.22E-03 1.44E-01 0 -3.61E-01
eq
ADPE kg Sb eq 1.61E-05 9.75E-07 2.21E-08 0 2.32E-07 2.81E-06 0 -5.53E-05
ADPF MJ 2.07E+03 1.44E+03 2.38E+00 0 3.02E+01 2.82E+02 0 -6.14E+03
m3 world eq
WDP 3.73E+01 1.3E-01 8.12E-01 0 2.58E-02 1.16E+02 0 -3.85E+01
deprived
GWP = Global warming potential; ODP = Depletion potential of the stratospheric ozone layer; AP = Acidification potential of land and water; EP =
Eutrophication potential; POCP = Formation potential of tropospheric ozone photochemical oxidants; ADPE = Abiotic depletion potential for non-fossil
resources; ADPF = Abiotic depletion potential for fossil resources; WDP = Water (user) deprivation potential)
RESULTS OF THE LCA - INDICATORS TO DESCRIBE RESOURCE USE according to EN 15804+A2: 1 m3 Sapelli finger-
jointed/laminated scantling
Parameter Unit A1-A3 A4 A5 C1 C2 C3 C4 D
PERE MJ 3.17E+04 8.19E-01 5.36E+01 0 2.1E+00 1.12E+04 0 -1.69E+03
PERM MJ 1.11E+04 0 -5.31E+01 0 0 -1.11E+04 0 0
PERT MJ 4.29E+04 8.19E-01 5.09E-01 0 2.1E+00 8.2E+01 0 -1.69E+03
PENRE MJ 2.03E+03 1.44E+03 5.02E+01 0 3.03E+01 2.82E+02 0 -6.14E+03
PENRM MJ 4.78E+01 0 -4.78E+01 0 0 0 0 0
PENRT MJ 2.07E+03 1.44E+03 2.38E+00 0 3.03E+01 2.82E+02 0 -6.14E+03
SM kg 2.79E-02 0 0 0 0 0 0 0
RSF MJ 0 0 0 0 0 0 0 0
NRSF MJ 0 0 0 0 0 0 0 0
FW m3 1.69E+00 4.26E-03 1.91E-02 0 2.42E-03 2.74E+00 0 -1.62E+00
PERE = Use of renewable primary energy excluding renewable primary energy resources used as raw materials; PERM = Use of renewable primary
energy resources used as raw materials; PERT = Total use of renewable primary energy resources; PENRE = Use of non-renewable primary energy
excluding non-renewable primary energy resources used as raw materials; PENRM = Use of non-renewable primary energy resources used as raw
materials; PENRT = Total use of non-renewable primary energy resources; SM = Use of secondary material; RSF = Use of renewable secondary fuels;
NRSF = Use of non-renewable secondary fuels; FW = Use of net fresh water
RESULTS OF THE LCA – WASTE CATEGORIES AND OUTPUT FLOWS according to EN 15804+A2:
1 m3 Sapelli finger-jointed/laminated scantling
Parameter Unit A1-A3 A4 A5 C1 C2 C3 C4 D
HWD kg 6.77E-08 3.55E-10 1.9E-10 0 1.61E-10 2.67E-08 0 -8.31E-07
NHWD kg 3.22E+00 9.01E-03 2.73E-01 0 4.94E-03 8.04E+00 0 -3.06E+00
RWD kg 7.55E-03 5.9E-05 1.07E-04 0 5.63E-05 2.19E-02 0 -4.84E-01
4 Environmental Product Declaration - Olam Agri - Sapelli finger-jointed/laminated scantlings
CRU kg 0 0 0 0 0 0 0 0
MFR kg 2.34E+02 0 1.92E-01 0 0 0 0 0
MER kg 0 0 0 0 0 0 0 0
EEE MJ 0 0 1.26E+01 0 0 1.61E+03 0 0
EET MJ 0 0 2.26E+01 0 0 2.89E+03 0 0
HWD = Hazardous waste disposed; NHWD = Non-hazardous waste disposed; RWD = Radioactive waste disposed; CRU = Components for re-use;
MFR = Materials for recycling; MER = Materials for energy recovery; EEE = Exported electrical energy; EET = Exported thermal energy
RESULTS OF THE LCA – additional impact categories according to EN 15804+A2-optional:
1 m3 Sapelli finger-jointed/laminated scantling
Parameter Unit A1-A3 A4 A5 C1 C2 C3 C4 D
Disease
PM 2.42E-03 3.12E-05 7.84E-09 0 1.77E-08 8.27E-07 0 -3.95E-06
incidence
IR kBq U235 eq 9.19E-01 5.03E-03 1.65E-02 0 8.51E-03 3.63E+00 0 -8.19E+01
ETP-fw CTUe 2.59E+03 4E+02 1.39E+00 0 2.14E+01 1.24E+02 0 -1.35E+03
HTP-c CTUh 8.29E-06 6.57E-09 7.61E-11 0 4.42E-10 7.59E-09 0 -6.21E-08
HTP-nc CTUh 6.22E-05 2.43E-07 5.24E-09 0 2.39E-08 2.66E-07 0 -2.38E-06
SQP SQP 5.39E+05 5.78E-01 5.8E-01 0 1.28E+01 8.69E+01 0 -1.1E+03
PM = Potential incidence of disease due to PM emissions; IR = Potential Human exposure efficiency relative to U235; ETP-fw = Potential comparative
Toxic Unit for ecosystems; HTP-c = Potential comparative Toxic Unit for humans (cancerogenic); HTP-nc = Potential comparative Toxic Unit for humans
(not cancerogenic); SQP = Potential soil quality index
Disclaimer 1 – for the indicator “Potential Human exposure efficiency relative to U235”. This impact category deals mainly with the
eventual impact of low-dose ionizing radiation on human health of the nuclear fuel cycle. It does not consider effects due to possible
nuclear accidents, occupational exposure or radioactive waste disposal in underground facilities. Potential ionizing radiation from the
soil, radon and from some construction materials is also not measured by this indicator.
Disclaimer 2 – for the indicators “abiotic depletion potential for non-fossil resources”, “abiotic depletion potential for fossil resources”,
“water (user) deprivation potential, deprivation-weighted water consumption”, “potential comparative toxic unit for ecosystems”,
“potential comparative toxic unit for humans – cancerogenic”, “Potential comparative toxic unit for humans - not cancerogenic”,
“potential soil quality index”. The results of this environmental impact indicator shall be used with care as the uncertainties on these
results are high as there is limited experience with the indicator.
This EPD was created using a software tool.
References
Standards version 2022.1
EN 15804 GaBi documentation
EN 15804:2012+A2:2019+AC:2021, Sustainability of GaBi dataset documentation for the software system and
construction works — Environmental Product Declarations — databases, LBP, University of Stuttgart and Sphera Solutions
Core rules for the product category of construction products. GmbH, Leinfelden-Echterdingen, 2021.
(http://www.gabi-software.com/support/gabi/gabi[1]database-
ISO 14025 2021-lci-documentation/)
EN ISO 14025:2011, Environmental labels anddeclarations —
Type III environmental declarations — Principles and PCR Part A
procedures. PCR - Part A: Calculation rules for the Life Cycle Assessment
Further References IBU 2021 and Requirements on the Background Report, version 1.3 from
Institut Bauen und Umwelt e.V.: General Instructions for the 08.2022, Institut Bauen und Umwelt e.V., www.bau-umwelt.com
EPD programme of Institut Bauen und Umwelt e.V., Version
2.0, Berlin: Institut Bauen und Umwelt e.V., 2021 www.ibu- PCR Part B
epd.com Part B: Requirements on the EPD for Solid wood product,
version from 08.2021
GaBi
GaBi Software System and Database for Life TROPIX
CycleEngineering, 1992-2021, Sphera Solutions GmbH, Fiche de l'essence Sapelli, TROPIX database, available at:
Leinfelden-Echterdingen, with acknowledgement of LBP https://tropix.cirad.fr/FichiersComplementaires/EN/Africa/SAPELLI.pdf
Verified EPD Tool
University of Stuttgart, program version GaBi 10; database CIB Solid wood products LCA-Tool - version 1.0
5 Environmental Product Declaration - Olam Agri - Sapelli finger-jointed/laminated scantlings
Publisher
Institut Bauen und Umwelt e.V. +49 (0)30 3087748- 0
Hegelplatz 1 info@ibu-epd.com
10117 Berlin www.ibu-epd.com
Germany
Programme holder
Institut Bauen und Umwelt e.V. +49 (0)30 3087748- 0
Hegelplatz 1 info@ibu-epd.com
10117 Berlin www.ibu-epd.com
Germany
Author of the Life Cycle Assessment
Olam Agri - Congolaise Industrielle des Bois +41612053944
Pokola BP 41 crs.congo@olamagri.com
BP 41 Ouesso www.olamagri.com
(Others)
Owner of the Declaration
Olam Agri - Congolaise Industrielle des Bois +41612053944
Pokola BP 41 crs.congo@olamagri.com
BP 41 Ouesso www.olamagri.com
(Others)
6 Environmental Product Declaration - Olam Agri - Sapelli finger-jointed/laminated scantlings
