ENVIRONMENTAL PRODUCT DECLARATION
as per ISO 14025 and EN 15804+A2
Owner of the Declaration Shaw Contract (Shaw Europe Ltd.)
Publisher Institut Bauen und Umwelt e.V. (IBU)
Programme holder Institut Bauen und Umwelt e.V. (IBU)
Declaration number EPD-SHA-20230441-CBA1-EN
Issue date 06.11.2023
Valid to 05.11.2028
EcoWorx S™ Carpet Tile with EcoSolution Q®, Solution Q®, or
Solution Q Extreme® Face Fibre
Shaw Contract (Shaw Europe Ltd.)
www.ibu-epd.com | https://epd-online.com
General Information
Shaw Contract (Shaw Europe Ltd.) EcoWorx S™ Carpet Tile with EcoSolution Q®,
Solution Q®, or Solution Q Extreme® Face Fibre
Programme holder Owner of the declaration
IBU – Institut Bauen und Umwelt e.V. Shaw Contract (Shaw Europe Ltd.)
Hegelplatz 1 Blackaddie Road *
10117 Berlin DG46DB Sanquhar
Germany United Kingdom
Declaration number Declared product / declared unit
EPD-SHA-20230441-CBA1-EN 1 m2 of installed EcoWorx STM Carpet Tile
This declaration is based on the product category rules: Scope:
Floor coverings, 01.08.2021 A Life Cycle Assessment (LCA) was conducted based upon production
(PCR checked and approved by the SVR) data collected from Shaw Contract (Shaw Europe, Ltd.), Plant SQ
manufacturing facility (Blackaddie Road, Sanquhar, DG46DB), located in
Scotland, UK. Production data was collected for EcoWorx STM Carpet Tile
Issue date with EcoSolution Q®, Solution Q®, or Solution Q Extreme® Face Fibre, for
06.11.2023 the period of one year, from January to December 2021.
This EPD is cradle-to-gate with options in scope with additional modules
Valid to A4, A5, B1 and B2. The EPD is created in accordance to the specifications
of EN 15804+A2.
05.11.2028
The functional unit has been defined as 1 m2 of installed EcoWorx STM
Carpet Tile.
The EPD was generated with the help of Envision LCA Tool, version 1. The
tool has not been manipulated in calculating impact results. The current
version of the tool is maintained, saved, and stored for 10 years to be used
for revision and re-traceability purposes.
The owner of the declaration shall be liable for the underlying information
and evidence; the IBU shall not be liable with respect to manufacturer
information, life cycle assessment data and evidences.
Dipl.-Ing. Hans Peters The EPD was created according to the specifications of EN 15804+A2. In
(Chairman of Institut Bauen und Umwelt e.V.) the following, the standard will be simplified as EN 15804.
Verification
The standard EN 15804 serves as the core PCR
Independent verification of the declaration and data according to ISO
14025:2011
internally X externally
Florian Pronold Mrs Kim Allbury,
(Managing Director Institut Bauen und Umwelt e.V.) (Independent verifier)
Environmental Product Declaration - Shaw Contract (Shaw Europe Ltd.) - EcoWorx S™ Carpet Tile with EcoSolution Q®, Solution Q®, or Solution Q Extreme® Face
1 Fibre
Product
Name Value Unit
Product description/Product definition
Product thickness 6 - 8 mm
This EPD applies to carpet tile with EcoWorx STM backing
Grammage 2719 g/m2
system together with EcoSolution Q®, Solution Q®, or Solution
Q Extreme® Nylon face fibre. Product Form Carpet Tile -
Yarn type - Solution-dyed 1% Post-industrial
-
EcoWorx STM is a commercial carpet tile, for use as a floor Nylon 6 Recycled Content
covering in accordance with manufacturer's guidelines. Total thickness 6 - 8 mm
Total carpet weight 2718 g/m2
The carpet tile consists of Shaw's unique face fibre, Nylon 6,
Surface pile thickness 1.2 - 3.4 mm
manufactured with 1% recycled material on the EcoWorx STM
Surface pile weight - Nominal
backing system, a polyolefin-based compound which is lighter 576 - 949 g/m2
Pile Mass
than traditional backings but offers superior durability and
Length and width of squared
strength. 250 - 1000 mm
elements
The EcoSolution Q®, Solution Q®, or Solution Q Extreme® face Other technical data parameters listed in IBU PCR Part B are
fibre is tufted into a primary backing sheet containing recycled not relevant and, therefore, have not been declared.
content. Latex is added to anchor the fibre and the EcoWorx
STM backing system is then applied. Performance data of the product in accordance with the
declaration of performance with respect to its essential
EcoWorx STM is suitable for use in all commercial settings. It characteristics according to 14041:2004A/C:2006.
has a life span of 15 years, and it comes with a 15-year
Base materials/Ancillary materials
warranty (subject only to installation and maintenance being
carried out in line with manufacturer's guidelines). EcoWorx STM Carpet Tile with EcoSolution Q®, Solution Q®, or
Solution Q Extreme® Face Fibre is comprised of the following
This product meets both internal and external performance raw materials:
standards including those established in the EU under EN 1307 • 30-35% Calcium Carbonate, containing Recycled
and EN 10874 for a product suitable for heavy and general Content
commercial installations. • 20-22% Polypropylene
For the placing on the market of the product in the European • 24-26% Solution-dyed Nylon 6 Face Fibre, containing
Union/European Free Trade Association (EU/EFTA) (with the 1% Post-industrial Recycled Content
exception of Switzerland) Regulation (EU) No. 305/2011 (CPR) • 3-5% Polyester Primary & Secondary Backing
applies. The product needs a declaration of performance taking • 1-3% Fibreglass Reinforcement
into consideration EN 14041:2004A/C:2006, and the CE- • 0-0.5% Anti-stat
marking. • 8.5-22% Proprietary Raw Materials
The product is packaged in cardboard boxes, wrapped in
For the application and use, the respective national provisions plastic, and stacked on wooden pallets for distribution.
apply.
The product fits into the defined scope and all raw material
Application
inputs, with no exceptions, are captured by the Envision LCA
EcoWorx STM Carpet Tile with EcoSolution Q®, Solution Q®, or
Tool, version 1.
Solution Q Extreme® Face Fibre is suitable for use as a floor
covering in heavy and general commercial installations. This product contains substances listed in the candidate list
(date: 17.01.2023) exceeding 0.1 percentage by mass: no
Technical Data
The technical specifications of the product are listed on the
This product contains other CMR substances in categories 1A
product's specification sheet, found at www.shawcontract.com.
or 1B which are not on the candidate list, exceeding 0.1
This product meets the requirements of the harmonized
percentage by mass: no
European Norm (hEN): EN14041:2004A/C:2006. Declarations
of performance related to fire, electrostatic, formaldehyde
Biocide products were added to this construction product or it
emissions, and slip resistance can be found on the product's
has been treated with biocide products (this then concerns a
specification sheet.
treated product as defined by the (EU) Ordinance on Biocide
Constructional data Products No. 528/2012): no
Reference service life
When properly installed as a commercial floor covering,
EcoWorx STM with EcoSolution Q®, Solution Q®, or Solution Q
Extreme® face fibre has a reference service life of 15 years.
This carpet tile product comes with a 15-year warranty, subject
only to installation and maintenance being carried out in
accordance with the manufacturer's guidelines.
LCA: Calculation rules
The declaration refers to the declared unit of 1 m² of installed
Declared Unit carpet tile.
Environmental Product Declaration - Shaw Contract (Shaw Europe Ltd.) - EcoWorx S™ Carpet Tile with EcoSolution Q®, Solution Q®, or Solution Q Extreme® Face
2 Fibre
• Module B5 - Refurbishment (module not relevant).
Declared unit
• Module B6 - Operational Energy Use (module not
Name Value Unit
relevant).
Declared unit 1 m2 • Module B7 - Operational Water Use (module not
Grammage 2.719 kg/m2 relevant).
End of Life Stage:
Layer thickness 0.007 m
Three scenarios have been evaluated:
Scenario 1: the EcoWorx STM carpet is 100% disposed of in a
System boundary
landfill.
The type of EPD is Cradle-to-Gate with options modules C1–
Scenario 2: the EcoWorx STM carpet is 100% incinerated.
C4, module D, and additional modules. The additional modules
Scenario 3: 40% of EcoWorx STM carpets are incinerated and
are A4, A5, B1 and B2.
the remaining 60% are landfilled. This assumption is based on
the carpet disposal rates in Europe mentioned in the study
The modules considered in the life cycle assessment and
conducted by Deutsche Umwelthilfe in 2017 (Umwelthilfe,
environmental product declaration, based on the product's
2017) and the European Commission in 2013 (Commission,
entire life cycle, are described as follows:
2013).
Production Stage: • Module C1 - The carpet is de-constructed manually and
no additional environmental impact is caused.
• Module A1 - Provision of Raw Materials.
• Module C2 - Transport of the carpet waste to a landfill or
• Module A2 - Transport of Raw Materials.
to the municipal waste incineration plant.
• Module A3 - Manufacturing.
• Module C3 - Impacts from thermal treatment disposal
Construction/Installation Stage:
(C3/2 and C3/3).
• Module A4 - Transportation by truck of the product to the • Module C4 - Impacts from landfill disposal (C4/1 and
construction site in Europe. C4/3).
• Module A5 - Installation of the carpet, treatment of Module D includes benefits from energy recovery via treatment
cutting waste (landfill) and packaging waste (landfill, of packaging materials and incineration of carpets at their end
recycling, and incineration). The production of the of life (D/1, D/2 and D/3), as well as the burdens of balancing
amount of carpet that occurs as installation waste is the secondary material content in modules A1 and A3 via the
also included along with its transport to the place of net-scrap approach.
installation. Biogenic carbon that is stored in the wooden
pallets and cardboard (packaging) is released as carbon Geographic Representativeness
dioxide emissions into the air at the end of life in module Land or region, in which the declared product system is
A5. manufactured, used or handled at the end of the product´s
Use Stage: lifespan: Europe
• Module B1 - Indoor emissions of volatile organic
compounds (VOCs) during the first few months after
Comparability
installation.
Basically, a comparison or an evaluation of EPD data is only
• Module B2 - Carpet cleaning per year, including
possible if all the data sets to be compared were created
vacuuming (electricity consumption) and hot water
according to EN 15804 and the building context, respectively
cleaning (electricity and water consumption, as well as
the product-specific characteristics of performance, are taken
waste water treatment).
into account. The background database used for the creation of
• Module B3 - Repair (module not relevant).
the EPD: GaBi ts software, CUP 2022.2.
• Module B4 - Replacement (module not relevant).
LCA: Scenarios and additional technical information
for the installation of EcoWorx STM carpet tile and should be
Characteristic product properties of biogenic carbon
used in accordance with the manufacturer's guidelines.
Biogenic carbon is only present in packaging (wooden pallets Installation losses have been accounted for in module A5.
and cardboards). Assumed water content in wooden pallet Product losses are considered as 5%.
(packaging): 18%.
Information on describing the Biogenic Carbon Content at The packaging material treatment and disposal are also
factory gate considered in module A5 (landfill, recycling, and incineration)
and the resulting benefits from energy generation are included
Name ValueUnit
in module D. The quantity of wooden pallets used is 0.133 kg
Biogenic carbon content in accompanying kg
0.14 per m². Wooden pallets are assumed to be re-used 20 times
packaging C
before being disposed of. Hence, the quantity of pallet disposed
is 0.007 kg. The quantity of cardboard packaging is 0.21 kg/m²
The following technical scenario information is required for the and the quantity of plastic packaging is 0.0103 kg/m². Total
declared modules and optional for non-declared modules. amount of packaging disposed at installation is 0.227 kg.
Packaging disposal rates (Source: Eurostat, Recovery and
Transport to the construction site (A4)
recycling rates for packaging).
Name Value Unit
• Paper - 82.8% recycled; 9.4% landfilled; and 7.8%
Transport distance (truck) 687 km
incinerated
Capacity utilisation (including empty runs) 55 %
• Plastic - 40.3% recycled; 28.7% landfilled; and 31.0%
incinerated
Installation in the building (A5)
• Wood pallets - 39.8% recycled; 34.5% landfilled; and
The installation of EcoWorx STM is done manually and no 25.7% incinerated
energy is required. A Pressure-Sensitive adhesive is required
Environmental Product Declaration - Shaw Contract (Shaw Europe Ltd.) - EcoWorx S™ Carpet Tile with EcoSolution Q®, Solution Q®, or Solution Q Extreme® Face
3 Fibre
Name ValueUnit End of Life (C1-C4)
Auxiliary 0.23 kg C1 - The product dismantling from the building is done
Material loss 0.136 kg manually without energy burden.
Output substances following waste treatment on C2 - Transportation of the product to the end of life is assumed
0.227 kg
site (packaging materials) to be 161 km (100 miles).
C3/2 - The EcoWorx STM carpet is 100% combusted in an
Use (B1) see cap. 2.12 use incineration plant with energy recovery (R>0.6).
Name Value Unit C3/3 - It is assumed that 40% of EcoWorx STM carpets are
Emissions to air (TVOC) after 50 days - Indoor Air incinerated and the remaining 60% are landfilled.
Comfort Gold® 900 mg/m² C4/1 - The EcoWorx STM carpet is 100% disposed of in landfill.
C4/3 - It is assumed that 40% of EcoWorx STM carpets are
Emission testing was conducted in accordance to Eurofins
incinerated and the remaining 60% are landfilled.
Indoor Air Comfort Gold® certification. After 28 days, the
Name ValueUnit
specific concentration of TVOCs was <100 ug/m3, as required
by the certification standard. Collected as mixed construction waste 2.719 kg
Landfilling (Scenario 1 - C3/1, C4/1 and D/1) 2.719 kg
Maintenance (B2) Incineration (Scenario 2 - C3/2, C4/2, and D/2) 2.719 kg
For the maintenance of EcoWorx STM Carpet Tile, 2 hot water Landfilling (60%) and Incineration (40%) (Scenario 2.719 kg
extraction cleanings (water and electricity consumption) per 3 - C3/3, C4/3 and D/3)
year as well as 52 vacuum cleanings (electricity consumption)
per year are recommended. The Reference Service Life of the Reuse, recovery and/or recycling potentials (D), relevant
product is 15 years. The results in the EPD declare a scenario information
maintenance for the period of 1 year. For the thermal and electrical energy generated in Module A5
Name Value Unit due to thermal treatment of packaging, avoided burdens have
Water consumption (1 year) 0.0009 m3 been calculated by the inversion of electricity grid mix and
thermal energy from natural gas, using European datasets.
Electricity consumption (1 year) 0.772 kWh
Module D also includes the environmental burdens linked to the
supply to secondary materials (nylon and calcium carbonate)
Reference service life
used in the carpet production.
Name ValueUnit
Reference service life (according to ISO 15686-1, -
15 a
2, -7 and -8)
Life Span according to the manufacturer 15 a
Environmental Product Declaration - Shaw Contract (Shaw Europe Ltd.) - EcoWorx S™ Carpet Tile with EcoSolution Q®, Solution Q®, or Solution Q Extreme® Face
4 Fibre
LCA: Results
The B2 module declares the maintenance (cleaning) per one year. The user of the EPD will be able to scale the results for its entire
useful life by multiplying the impact by the RSL.
The LCA results presented below applies to 100% landfilled end of life scenario.
DESCRIPTION OF THE SYSTEM BOUNDARY (X = INCLUDED IN LCA; MND = MODULE OR INDICATOR NOT DECLARED; MNR
= MODULE NOT RELEVANT)
Benefits and
Construction loads beyond
Product stage Use stage End of life stage
process stage the system
boundaries
la ire ta m w a Ry lp p u s tro p s n a rT g n iru tc a fu n a M e h t m o rf tro p s n a rTe tis e h t o t e ta g y lb m e s s A e s U e c n a n e tn ia M ria p e R tn e m e c a lp e R tn e m h s ib ru fe R y g re n e la n o ita re p Oe s u re ta w la n o ita re p Oe s u n o itc u rts n o c -e Dn o itilo m e d tro p s n a rT g n is s e c o rp e ts a W la s o p s iD -e s u e R-y re v o c e R-g n ilc y c e Rla itn e to p
A1 A2 A3 A4 A5 B1 B2 B3 B4 B5 B6 B7 C1 C2 C3 C4 D
X X X X X X X MNR MNR MNR MND MND X X X X X
RESULTS OF THE LCA - ENVIRONMENTAL IMPACT according to EN 15804+A2: 1 m² EcoWorx S™ Carpet
Parameter Unit A1-A3 A4 A5 B1 B2 C1 C2 C3 C4 D
GWP-total kg CO 2 eq 8.68E+00 1.77E-01 5.54E-01 2.54E-04 2.89E-01 0 3.68E-02 0 1.91E-01 3.98E-02
GWP-fossil kg CO 2 eq 9.01E+00 1.76E-01 5.58E-01 2.54E-04 2.86E-01 0 3.67E-02 0 1.93E-01 3.57E-02
GWP-
biogenic kg CO 2 eq -3.39E-01 -2.43E-04 -4.19E-03 0 3.05E-03 0 -5.07E-05 0 -2.05E-03 4.11E-03
GWP-luluc kg CO 2 eq 2.74E-03 9.81E-04 2.3E-04 0 6.06E-05 0 2.05E-04 0 9.38E-05 1.14E-05
ODP kg CFC11 eq 8.28E-09 1.05E-14 4.36E-10 0 4.19E-12 0 2.2E-15 0 2.59E-13 1.87E-14
AP mol H+ eq 2.53E-02 1.81E-04 1.73E-03 0 6.29E-04 0 3.78E-05 0 5.71E-04 7.57E-05
EP-
kg P eq 1.92E-05 5.25E-07 1.48E-05 0 1.4E-06 0 1.1E-07 0 3.6E-05 3E-08
freshwater
EP-marine kg N eq 7.08E-03 5.93E-05 4.43E-04 0 1.43E-04 0 1.24E-05 0 1.26E-04 2.43E-05
EP-terrestrial mol N eq 7.19E-02 7.06E-04 5.19E-03 0 1.48E-03 0 1.47E-04 0 1.39E-03 2.05E-04
kg NMVOC
POCP 2.2E-02 1.6E-04 1.48E-03 1.41E-05 3.82E-04 0 3.33E-05 0 4.06E-04 7.39E-05
eq
ADPE kg Sb eq 4.01E-06 1.47E-08 2.36E-07 0 7.8E-08 0 3.07E-09 0 1.34E-08 2.53E-09
ADPF MJ 1.99E+02 2.35E+00 1.17E+01 0 5.19E+00 0 4.9E-01 0 2.73E+00 6.29E-01
m3 world eq
WDP 1.03E+00 1.58E-03 1.24E-01 0 6.54E-02 0 3.29E-04 0 -1.9E-03 -1.32E-03
deprived
GWP = Global warming potential; ODP = Depletion potential of the stratospheric ozone layer; AP = Acidification potential of land and water; EP =
Eutrophication potential; POCP = Formation potential of tropospheric ozone photochemical oxidants; ADPE = Abiotic depletion potential for non-fossil
resources; ADPF = Abiotic depletion potential for fossil resources; WDP = Water (user) deprivation potential)
RESULTS OF THE LCA - INDICATORS TO DESCRIBE RESOURCE USE according to EN 15804+A2: 1 m² EcoWorx S™ Carpet
Parameter Unit A1-A3 A4 A5 B1 B2 C1 C2 C3 C4 D
PERE MJ 1.05E+01 1.41E-01 5.1E+00 0 2.88E+00 0 2.79E-02 0 2.25E-01 -5.35E-02
PERM MJ 5.31E+00 0 -4.19E+00 0 0 0 0 0 0 0
PERT MJ 1.58E+01 1.41E-01 9.16E-01 0 2.88E+00 0 2.79E-02 0 2.25E-01 -5.35E-02
PENRE MJ 1.62E+02 2.48E+00 1.51E+00 0 5.19E+00 0 4.91E-01 0 2.74E+00 6.3E-01
PENRM MJ 5.16E+01 0 -3.17E-01 0 0 0 0 0 0 0
PENRT MJ 2.12E+02 2.48E+00 1.19E+00 0 5.19E+00 0 4.91E-01 0 2.74E+00 6.3E-01
SM kg 7.85E-01 0 4.13E-02 0 0 0 0 0 0 -8.26E-01
RSF MJ 0 0 0 0 0 0 0 0 0 0
NRSF MJ 0 0 0 0 0 0 0 0 0 0
FW m3 3.64E-02 1.51E-04 9.98E-03 0 2.75E-03 0 3.15E-05 0 3.54E-05 4.11E-06
PERE = Use of renewable primary energy excluding renewable primary energy resources used as raw materials; PERM = Use of renewable primary
energy resources used as raw materials; PERT = Total use of renewable primary energy resources; PENRE = Use of non-renewable primary energy
excluding non-renewable primary energy resources used as raw materials; PENRM = Use of non-renewable primary energy resources used as raw
materials; PENRT = Total use of non-renewable primary energy resources; SM = Use of secondary material; RSF = Use of renewable secondary fuels;
NRSF = Use of non-renewable secondary fuels; FW = Use of net fresh water
RESULTS OF THE LCA – WASTE CATEGORIES AND OUTPUT FLOWS according to EN 15804+A2:
1 m² EcoWorx S™ Carpet
Parameter Unit A1-A3 A4 A5 B1 B2 C1 C2 C3 C4 D
HWD kg 1.02E-08 1.13E-11 2.97E-09 0 4.49E-10 0 2.35E-12 0 4.22E-10 6.92E-11
NHWD kg 2.81E-01 3.38E-04 1.86E-01 0 4.77E-03 0 7.04E-05 0 2.71E+00 -8.1E-05
RWD kg 4.35E-03 2.9E-06 2.48E-04 0 8.3E-04 0 6.05E-07 0 3.36E-05 -1.12E-05
CRU kg 0 0 0 0 0 0 0 0 0 0
Environmental Product Declaration - Shaw Contract (Shaw Europe Ltd.) - EcoWorx S™ Carpet Tile with EcoSolution Q®, Solution Q®, or Solution Q Extreme® Face
5 Fibre
MFR kg 0 0 1.81E-01 0 0 0 0 0 0 0
MER kg 0 0 0 0 0 0 0 0 0 0
EEE MJ 0 0 6.37E-02 0 0 0 0 0 0 0
EET MJ 0 0 9.77E-02 0 0 0 0 0 0 0
HWD = Hazardous waste disposed; NHWD = Non-hazardous waste disposed; RWD = Radioactive waste disposed; CRU = Components for re-use;
MFR = Materials for recycling; MER = Materials for energy recovery; EEE = Exported electrical energy; EET = Exported thermal energy
RESULTS OF THE LCA – additional impact categories according to EN 15804+A2-optional:
1 m² EcoWorx S™ Carpet
Parameter Unit A1-A3 A4 A5 B1 B2 C1 C2 C3 C4 D
Disease
PM 2.5E-07 1.05E-09 1.79E-08 0 5.21E-09 0 2.18E-10 0 5.49E-09 5.33E-09
incidence
IR kBq U235 eq 4.13E-01 4.26E-04 2.42E-02 0 1.41E-01 0 8.87E-05 0 4.96E-03 -9.14E-04
ETP-fw CTUe 9.11E+01 1.63E+00 5.75E+00 1.15E-04 2.35E+00 0 3.4E-01 0 2.68E+00 3.17E-01
HTP-c CTUh 2.1E-09 3.29E-11 1.44E-10 0 6.79E-11 0 6.86E-12 0 1.2E-10 9.5E-12
HTP-nc CTUh 6.8E-08 1.71E-09 5.56E-09 3.07E-12 2.65E-09 0 3.56E-10 0 1.01E-08 3.68E-10
SQP SQP 1.22E+01 8.1E-01 1.1E+01 0 1.87E+00 0 1.69E-01 0 1.97E-01 -5.84E-01
PM = Potential incidence of disease due to PM emissions; IR = Potential Human exposure efficiency relative to U235; ETP-fw = Potential comparative
Toxic Unit for ecosystems; HTP-c = Potential comparative Toxic Unit for humans (cancerogenic); HTP-nc = Potential comparative Toxic Unit for humans
(not cancerogenic); SQP = Potential soil quality index
Disclaimer 1: For the indicator 'Potential Human exposure efficiency relative to U235". This impact category deals mainly with the
eventualimpact of low dose ionizing radiation on human health of the nuclear fuelcycle. It does not consider effects due to possible
nuclear accidents, occupationalexposure nor due to radioactive waste disposal in underground facilities.Potential ionizing radiation
from the soil, from radon and from someconstruction materials is also not measured by this indicator.
Disclaimer 2: For the indicators 'Abiotic depletionpotential for non-fossil resources', “Abiotic depletion potential for fossilresources”,
“Water (user) deprivation potential","Deprivation-weighted water consumption”, “Potential comparative toxicunit for ecosystems”,
“Potential comparative toxic unit for humans -cancerogenic”, “Potential comparative toxic unit for humans -non-carcinogenic”, “Potential
soil quality index”. The results of theseenvironmental impact indicators shall be used with care as the uncertainties onthese results are
high or as there is limited experienced with the indicators. This EPD was created using a software tool.
References
STANDARDS: life planning — Part 2: Service life prediction procedures.
EN 10874 ISO 15686
EN 10874:2009, Resilient, textile and laminate floor coverings ISO 15686-7:2011, Building and constructed assets — Service
— Classification. life planning — Part 7: Performance evaluation for feedback of
service life data from practice.
EN 1307
EN 1307:2014, Textile floor coverings — Classification. ISO 15686
ISO 15686-8:2011, Building and constructed assets — Service
EN 14041 life planning — Part 8: Reference service life and service life
EN 14041:2004/AC:2006 — Resilient, textile and laminate floor estimation.
coverings — Essential characteristics.
FURTHER REFERENCES:
EN 15804
EN 15804:2012+A2:2019/AC:2021, Sustainability of Candidate list
construction works — Environmental product declarations — Candidate List of substances of very high concern for
Core rules for the product category of construction products. Authorisation, published on ECHA website, latest version
17.01.2023 (https://echa.europa.eu/candidatelist-table).
ISO 14025
ISO 14025:2011, Environmental labels and declarations — Deutsche Umwelthilfe
Type III environmental declarations — Principles and Deutsche Umwelthilfe. Swept under the Carpet: The Big Waste
procedures. Problem of the Carpet Industry in Germany, 2017.
ISO 14040 Envision LCA Tool
ISO 14040:2006, Environmental management — Life cycle Envision LCA Tool, 2021, Sphera Solutions GmbH, Leinfelden-
assessment — Principles and framework. Echterdingen, with acknowledgement of LBP University of
Stuttgart, version 1.
ISO 14044
ISO 14044:2006, Environmental management — Life cycle GaBi
assessment — Requirements and guidelines. GaBi Software System and Database for Life Cycle
Engineering, 1992-2021, Sphera Solutions GmbH, Leinfelden-
ISO 15686 Echterdingen, with acknowledgement of LBP University of
ISO 15686-1:2011, Building and constructed assets — Service Stuttgart, program version GaBi 10; database version 2021.1.
life planning — Part 1: General principles and framework.
GaBi documentation
ISO 15686 GaBi dataset documentation for the software system and
ISO 15686-2:2011, Building and constructed assets — Service databases, LBP, University of Stuttgart and Sphera Solutions
Environmental Product Declaration - Shaw Contract (Shaw Europe Ltd.) - EcoWorx S™ Carpet Tile with EcoSolution Q®, Solution Q®, or Solution Q Extreme® Face
6 Fibre
GmbH, Leinfelden-Echterdingen, 2021 (http://www.gabi-
software.com/support/gabi/gabi-database-2021-lci- PCR Part B
documentation/). Product Category Rules for Building Products, Part B:
Requirements on the EPD for floor coverings, version 1.7, 2022
IBU 2021 (www.bau-umwelt.de).
Institut Bauen und Umwelt e.V.: General Instructions for the
EPD programme of Institut Bauen und Umwelt e.V., Version Packaging disposal rates
2.0, Berlin: Institut Bauen und Umwelt e.V., 2021 (www.ibu- Eurostat, Recovery and recycling rates for packaging. 2015
epd.com). (http://ec.europa.eu/eurostat/web/environment/waste/main-
tables).
PCR Part A The literature referred to in the Environmental Product
PCR Part A: Calculation rules for the Life Cycle Assessment Declaration must be listed in full.Standards already fully quoted
and Requirements on the Background Report according to EN in the EPD do not need to be listed here again.
15804:2012+A2:2019/AC:2021, Version 1.3, Institut Bauen und The current version of PCR Part A and PCR Part B of the PCR
Umwelt e.V., 2021. document on which they are based must be referenced.
Environmental Product Declaration - Shaw Contract (Shaw Europe Ltd.) - EcoWorx S™ Carpet Tile with EcoSolution Q®, Solution Q®, or Solution Q Extreme® Face
7 Fibre
Publisher
Institut Bauen und Umwelt e.V. +49 (0)30 3087748- 0
Hegelplatz 1 info@ibu-epd.com
10117 Berlin www.ibu-epd.com
Germany
Programme holder
Institut Bauen und Umwelt e.V. +49 (0)30 3087748- 0
Hegelplatz 1 info@ibu-epd.com
10117 Berlin www.ibu-epd.com
Germany
Author of the Life Cycle Assessment
Sphera Solutions GmbH +49 711 341817-0
Hauptstraße 111- 113 info@sphera.com
70771 Leinfelden-Echterdingen www.sphera.com
Germany
Owner of the Declaration
Shaw Contract (Shaw Europe Ltd.) +1 800 257 7429
Blackaddie Road * infouk@shawcontract.com
DG46DB Sanquhar www.shawcontract.com
United Kingdom
Environmental Product Declaration - Shaw Contract (Shaw Europe Ltd.) - EcoWorx S™ Carpet Tile with EcoSolution Q®, Solution Q®, or Solution Q Extreme® Face
8 Fibre
