ENVIRONMENTAL PRODUCT DECLARATION
as per ISO 14025 and EN 15804+A2
Owner of the Declaration DBC, EFCC, FEICA, IVK
Programme holder Institut Bauen und Umwelt e.V. (IBU)
Publisher Institut Bauen und Umwelt e.V. (IBU)
Declaration number EPD-FEI-20220109-IBG1-EN
Issue date 01.06.2022
Valid to 31.05.2027
Products based on polyurethane, group 5
DBC - Deutsche Bauchemie e.V.
EFCC - European Federation for Construction Chemicals
FEICA - Association of the European Adhesive and Sealant Industry
IVK - Industrieverband Klebstoffe e.V.
www.ibu-epd.com | https://epd-online.com
Umwelt Produktdeklaration Name des Herstellers – Name des Produkts
1. General Information
DBC - Deutsche Bauchemie e.V. Products based on polyurethane,
EFCC - European Federation for group 5
Construction Chemicals
FEICA - Association of the European
Adhesive and Sealant Industry
IVK - Industrieverband Klebstoffe e.V.
Programme holder Owner of the declaration
IBU – Institut Bauen und Umwelt e.V. DBC, Mainzer Landstr. 55, D-60329 Frankfurt a.M.
Hegelplatz 1 EFCC, 172 Boulevard du Triomphe, B-1160 Brussels
10117 Berlin FEICA, Rue Belliard 40, B-1040 Brussels
Germany IVK, Völklingerstr. 4, D-40219 Düsseldorf
Declaration number Declared product / declared unit
EPD-FEI-20220109-IBG1-EN 1 kg product based on polyurethane; density 0.85 -
1.8 g/cm³
This declaration is based on the product Scope:
category rules: This verified EPD entitles the holder to bear the symbol
Reaction resin products, 07.2014 of the Institut Bauen und Umwelt e.V. It exclusively
(PCR checked and approved by the SVR) applies for products produced in Europe and for a
period of five years from the date of issue. This EPD
may be used by members of DBC, EFCC, FEICA and
Issue date
IVK and their members provided it has been proven
01.06.2022
that the respective product can be represented by this
EPD. For this purpose a guideline is available at the
Valid to secretariats of the four associations. The members of
31.05.2027 the associations are listed on the respective websites.
The owner of the declaration shall be liable for the
underlying information and evidence; the IBU shall not
be liable with respect to manufacturer information, life
cycle assessment data and evidences.
The EPD was created according to the specifications
of EN 15804+A2. In the following, the standard will be
simplified as EN 15804.
Verification
The standard EN 15804 serves as the core PCR
Independent verification of the declaration and data
according to ISO 14025:2011
Dipl. Ing. Hans Peters internally x externally
(chairman of Institut Bauen und Umwelt e.V.)
Dr. Alexander Röder Matthias Schulz
(Managing Director Institut Bauen und Umwelt e.V.)) (Independent verifier)
2. Product
2.1 Product description/Product definition product for calculating the Life Cycle Assessment
This EPD comprises reactive products based on results (worst-case approach).
polyurethane (PU) with a volatile organic compound
(VOC) content ≤1 % (VOC definition according to For the placing on the market in the European
Decopaint Directive) and a castor oil/-derivatives Union/European Free Trade Association (EU/EFTA)
content ≥10 %. The one- or two-component reactive with the exception of Switzerland) products falling
PU products are manufactured using polyols and under Regulation (EU) No 305/2011 (CPR) need a
isocyanates. The aqueous systems consist of (a) Declaration of Performance taking into consideration
dispersion and are crosslinked by a dispersible either the relevant harmonised European standard or
isocyanate. The products fulfil manifold, often specific, the European Technical Assessment and the CE
functions in the construction, furnishing and repair of marking. For the application and use of the products
buildings. The product displaying the highest the respective national provisions apply.
environmental impacts was used as a representative
2 Environmental Product Declaration FEICA/EFCC/IVK/DBC – Products based on polyurethane, group 5
2.2 Application Installing mechanically fixed external windows and
Products based on polyurethane, group 5, are used for doors with an OCF, as part of a system including
the following applications: sealants and tapes
12.2 Door Installation & Fixation:
Module 1: Adhesives for parquet and floor Fixing interior doors with an OCF
coverings 12.3 General Gap Filling:
Parquet adhesives in accordance with EN ISO 17178 Filling of regularly and irregularly shaped spaces
for wooden and parquet floors and flooring adhesives between at least two surfaces made of typical building
in accordance with EN ISO 22636 for floor coverings materials with a one-component foam (OCF)
Module 2: Reactive products for protecting and Module 13: Sealants for glazing
repairing concrete structures Two-component reactive sealants are to be used as
Products for increasing the durability of concrete and the second barrier of the structural hermetic seal in
reinforced concrete structures as well as for new insulating glass units.
concrete and for maintenance and repair work
(requirements 2.1), products for structural bonding of Module 14: Bonded glazing sealants
strengthening materials to an existing concrete One- and two-component reactive sealants are used
structure (requirements 2.2) and products for concrete for the bonding of insulating glass units in the window
injection for filling cracks, voids and interstices in frame.
concrete (requirements 2.3)
2.3 Technical Data
Module 3: Liquid-applied roof waterproofing kits The density of the products is between 0,85 and 1,8
Reactive products for waterproofing roof constructions g/cm³, other relevant technical data can be found in the
which are applied on site manufacturer’s technical documentation.
Module 4: Reactive products for liquid-applied Module 1: Reactive products as adhesive for
bridge deck waterproofing kits parquet and floor coverings
Products for liquid-applied waterproofing for use on The minimum requirements of EN ISO 17178 and EN
concrete bridge decks ISO 22636 must be maintained.
Module 5: Screed material, floor screeds and Module 2: Reactive products for protecting and
decorative floors repairing concrete structures
Products for screed/synthetic resin screed for use in 2.1 The requirements on essential characteristics for
floor constructions all intended uses in accordance with EN 1504-2,
Tables 1 and 5 must be maintained. These are:
Module 6: Reactive products as an adhesive for - Permeability to CO (EN 1062-6)
2
tiles - Water vapour permeability (EN ISO 7783-1/-2)
Tile adhesives for internal and external tile installations - Capillary absorption and permeability to water (EN
on walls, floors and ceilings 1062-3)
- Adhesive strength by pull-off test (EN 1542)
Module 7: Adhesives and sealants 2.2 Essential characteristics for all intended uses in
Reactive products for use as: accordance with EN 1504-4, Tables 3.1 and 3.2
· Structural and repair adhesives (manufacturer's declaration of performance)
· Surface and joint sealants 2.3 Requirements on essential characteristics for all
Applications in accordance with the manufacturer's intended uses in accordance with EN 1504-5, Table 3:
technical documentation / declaration of performance - Injectability (EN 1771)
- Viscosity (EN ISO 3219)
Module 8: Reactive products for watertight Further essential characteristics in accordance with the
covering kits manufacturer's technical documentation / declaration
Products for waterproofing floors and/or walls in wet of performance
rooms inside buildings
Module 3: Liquid-applied roof waterproofing kits
Module 9: Reactive products for liquid-applied The minimum requirements of EAD 030350-00-0402
waterproofing Liquid-applied roof waterproofing kits must be
Liquid applied products for waterproofing of buildings maintained. The essential characteristics are to be
specified in accordance with the European Technical
Module 10: Reactive products for waterproofing Assessment (ETA, specification no.).
and/or for pre-treating mineral substrates
Applications in accordance with the manufacturer's Module 4: Reactive products for liquid-applied
technical documentation bridge deck waterproofing kits
The minimum requirements of ETAG 033 Liquid-
Module 11: Liquid-applied waterproofing applied bridge deck waterproofing kits must be
membranes for use beneath ceramic tiling maintained. The essential characteristics are to be
specified in accordance with the European Technical
Module 12: One-component foam (OCF) Assessment (ETA, specification no.).
One component foam in a can is a one-component,
self-expanding, ready to use polyurethane foam used Module 5: Screed material, floor screeds and
for various construction applications. It consists of a decorative floors
low viscous semi-fluid in a can that leaves the can as a The requirements on essential characteristics
froth and immediately forms a polyurethane foam. according to EN 13813 'Screed material and floor
12.1 Window & External Door Sealing & Insulation: screeds – Screed materials – Properties and
3 Environmental Product Declaration FEICA/EFCC/IVK/DBC – Products based on polyurethane, group 5
requirements'/ must be maintained. For synthetic resin tiling - Definitions, specifications and test methods-
screeds, these are: must be maintained. These are:
- Bond strength (EN 13892-8) - Initial tensile adhesion strength
- Reaction to fire (EN 13501-1) - Tensile adhesion strength after water contact
Further essential characteristics in accordance with the - Tensile adhesion strength after heat ageing
manufacturer's technical documentation/declaration of - Tensile adhesion strength after freeze-thaw cycles
performance - Waterproofing
- Crack bridging ability
Module 6: Reactive products as an adhesive for
tiles
Module 12: One-Component Foams
The requirements on essential characteristics
Physical data of the one-component foam must be
according to EN12004, must be maintained. These
indicated in accordance with the respective product
are:
standards; these can include, for example:
-Tensile adhesion strength after dry storage (EN
12004-2)
12.1 Window & External Door Sealing & Insulation
-Tensile adhesion strength after water immersion (EN
Tensile Strength EN 17333-4, Movement Capability
12004-2)
EN 17333-4, Curing Pressure EN 17333-2, Thermal
-Tensile adhesion strength after heat ageing (EN
conductivity EN 17333-5, Sound Insulation EN ISO
12004-2)
717-1, Post expansion EN 17333-2
-Tensile adhesion strength after freeze/thaw cycles
(EN 12004-2)
-Open time: Tensile strength (EN 12004-2) 12.2 Door Installation & Fixation
Further essential characteristics in accordance with the Shear Strength EN 17333-4, Tensile Strength
manufacturer's technical documentation EN 17333-4, Compression Strength EN 17333-4,
Curing pressure EN 17333-2
Module 7: Adhesives and sealants
Performance characteristics in accordance with the
12.3 General Gap Filling
manufacturer's technical documentation/declaration of
Sagging EN 17333-3 Other performance
performance
characteristics in accordance with the manufacturer's
technical documents/declaration of performance.
Module 8: Reactive products for watertight
covering kits
The minimum requirements of EAD 030352-00-0503 Module 13: Sealants for glazing
Liquid applied watertight covering kits for wet room Reactive sealants must comply with EN 1279-4
floors and/or walls must be maintained. The essential Performance characteristics in accordance with the
characteristics are to be specified in accordance with manufacturer's technical documentation/declaration of
the European Technical Assessment (ETA, performance
specification no.).
Module 14: Bonded glazing sealants
Module 9: Reactive products for liquid-applied Reactive sealants must comply with RAL-GZ 716 part
waterproofings 2 and ift-Guideline VE-08/4.
The minimum requirements of the test principles Performance characteristics in accordance with the
regarding the issuing of general building authority test manufacturer's technical documentation/declaration of
certificates for liquid-applied products for waterproofing performance
of buildings (PG-FLK) must be maintained. The
characteristics for the proof of usability are to be
specified in accordance with the test principles for
granting general building authority test certificates for
liquid applied polymer products for waterproofing
buildings
Module 10: Reactive products for waterproofing 2.4 Delivery status
and/or for pre-treating mineral substrates Liquid or pasty in containers made of tinplate or plastic
packed in separate or combi-containers for the
Name Value Unit required mixing ratio. Packages containing one kg of
Density acc. to EN ISO 2811-1 700 - 1800 kg/m3 product in different types of containers. Sealants in
Shore hardness A acc. to ISO 48- plastic cartridges and foil packs. Typical container
4 >15 sizes contain 10 to 25 kg of material. For major works,
Shore hardness D acc. to ISO 48- vats containing approx. 200 kg or IBCs (intermediate
4 >5 bulk containers) containing 1 tonne or more are also
used. The LCA is based on tinplate, plastic and wood
Viscosity acc. to ISO 3219-2 <100 Pas
packaging.
Other performance characteristics in accordance with
the manufacturer's technical
2.5 Base materials/Ancillary materials
documentation/declaration of performance
Products based on polyurethane with a VOC content
≤1 % and a castor oil/-derivatives content ≥10 %
Module 11: Liquid-applied waterproofing
usually comprise a reactive polymer and a crosslinking
membranes for use beneath ceramic tiling
system. The polymer component contains polyether
The minimum requirements on essential
and/or polyester polyols. Crosslinking takes place after
characteristics according to EN 14891 - Liquid applied
installation on site. In the case of two-component
water-impermeable products for use beneath ceramic
systems, this involves the use of pre-polymers and
4 Environmental Product Declaration FEICA/EFCC/IVK/DBC – Products based on polyurethane, group 5
polymers based on typically methylene diphenyl
diisocyanate (MDI), toluene diisocyanate (TDI), 2.7 Environment and health during
hexamethylene diisocyanate (HDI) or isophorone manufacturing
diisocyanate. The resin mixing ratio is adjusted As a general rule, no other environmental protection
according to the stoichiometric requirements. measures other than those specified by law are
Crosslinking starts directly after the components have necessary.
been mixed. There are also one-component reactive
polymer formulations based on PU which crosslink in 2.8 Product processing/Installation
the presence of moisture. They comprise prepolymers Products based on polyurethane, are processed by
based on e.g. MDI, TDI, HDI, IPDI. In formulations with trowelling/knife-coating or rolling, pouring, spraying or
aqueous dispersions, dispersible isocyanates are used injection.
for crosslinking. The formulations can contain auxiliary Precautions for safe handling and storage (e.g. air
materials such as accelerators, catalysts, wetting exchange, exhaust ventilation, personal protective
agents, foam regulators and viscosity regulators for measures, precautions required in the handling of
fine-tuning the product features. Typically, the isocyanates, conditions for safe storage) must be
products covered by this EPD contain the following observed in accordance with the information on the
ranges of base materials and auxiliaries: safety data sheet.
Polyol component: up to approx. 50 %
Crosslinking component: up to approx. 95 % 2.9 Packaging
Plasticiser: ~ 0-25 % A detailed description of packaging is provided in
Additives / Pigments: ~ 0-30 % section 2.4. Empty containers and clean foils can be
Water: ~ 0-60 % recycled.
VOC: ≤1 % according to the Decopaint Directive
(mandatory)
Castor oil and derivatives: ≥10 % (mandatory) 2.10 Condition of use
During the use phase, products based on polyurethane
These ranges are average values and the composition are crosslinked and essentially comprise an inert
of products complying with the EPD can deviate from three-dimensional network. They are long-lasting
these concentration levels in individual cases. More products which protect our buildings in the form of
detailed information is available in the respective adhesives, coatings or sealants as well as make an
manufacturer's documentation (e.g. product data essential contribution in retaining their function and
sheets). long-term value.
Note: For companies to declare their products within
the scope of this EPD it is not sufficient to simply 2.11 Environment and health during use
comply with the product composition shown above. Option 1: Products for applications outside indoor
The application of this EPD is only possible for areas with permanent stays by people
member companies of DBC, EFCC, FEICA, and IVK During use, the reactive products lose their reactive
member associations and only for specific formulations properties and become inert. No risks are known for
with a total score below the declared maximum score water, air and soil if the products are used as
for a product group according to the associated designated.
guidance document. Option 2: Products for applications inside indoor
areas with permanent stays by people
When used in indoor areas with permanent stays by
1. substances from the “Candidate List of people, evidence of the emission performance of
Substances of Very High Concern for construction products in contact with indoor air must be
Authorisation” (SVHC) submitted according to national requirements (see
If this product contains substances listed in the chapter 7). No further influences by emissions on the
candidate list (latest version) exceeding 0.1 environment and health are known.
percentage by mass, the relevant information can be
found in the safety data sheet of the relevant product
covered by this model EPD. 2.12 Reference service life
2. CMR substances in categories 1A and 1B Cured products based on polyurethane fulfil manifold,
If this product contains other carcinogenic, mutagenic, often specific functions in the construction or
reprotoxic (CMR) substances in categories 1A or 1B refurbishment of building structures. They decisively
which are not on the candidate list, exceeding 0.1 improve the usability of building structures and
percentage by mass, the relevant information can be significantly extend their original service lives. The
found in the safety data sheet of the relevant product anticipated reference service life depends on the
covered by this model EPD. specific installation situation and the exposure
3. Biocide products added to the construction associated with the product. It can be influenced by
product weathering as well as mechanical or chemical loads.
If this construction product contains biocide products,
the active substances, information on the
concentration and/or concentration range, the product 2.13 Extraordinary effects
type together with information on their hazardous
properties are listed in the safety data sheet of the Fire
respective product. Even without any special fire safety features, cured
products based on polyurethane comply with at least
the requirements of EN 13501-1 standard for fire
2.6 Manufacture classes E and Efl. In terms of the volumes applied,
The components of the formulation are usually mixed they have only a marginal influence on the fire
batch-wise and packaged for delivery. performance characteristics (e.g. smoke gas
5 Environmental Product Declaration FEICA/EFCC/IVK/DBC – Products based on polyurethane, group 5
development) of the building structure in which they not interfere with the disposal/recycling of the
have been installed. As crosslinked polyurethane remaining components/building materials.
systems do not melt or drip, they do not contribute
towards spreading fire. 2.15 Disposal
Residual material which cannot be used or recycled
Water must be combined at a specified ratio and hardened.
Cured reactive products based on polyurethane are Hardened product residue is not special waste. Non-
chemically inert and insoluble in water. They are often hardened product residue is hazardous waste. Empty,
used to protect building structures from harmful water dried containers (free of drops and scraped clean) are
ingress or the effects of flooding. directed to the recycling process. Residue must be
directed to proper waste disposal taking into
Mechanical destruction consideration the local guidelines. The following waste
Mechanical destruction of cured reactive products codes according to the European List of Waste
based on polyurethane does not lead to any (2000/532/EC) can apply:
decomposition products which are harmful to the Hardened product residue:
environment or health. European Waste Catalogue (EWC) code 080112
(waste paint and varnish with the exception of that
2.14 Re-use phase mentioned in 08 01 11)
According to present knowledge, no environmentally EWC code 080410 (waste adhesives and sealants
harmful effects are generally anticipated in landfilling, other than mentioned in 08 04 09)
for example, as a result of de-construction and
recycling of building materials with adherent 2.16 Further information
crosslinked products. If the crosslinked products can More information is available on the manufacturer's
be removed from construction products without large product or safety data sheets and on the
effort, thermal recovery is a practical recycling variant manufacturer's websites or on request. Valuable
on account of their energy content. Minor adhesion is technical information is also available on the
not taken into consideration during disposal. It does associations' websites.
3. LCA: Calculation rules
3.1 Declared Unit contain substances in the formulation that directly emit
This EPD refers to the declared unit of 1 kg of product (as) VOC, but VOCs are generated by a chemical
based on polyurethane, group 5; applied into the reaction that are occurring during this phase. The end
building with a density of 0.85 - 1.8 g/cm³ in of life for the packaging material considered is
accordance with the IBU PCR part B for reaction resin described below:
products. -Incineration, for materials like plastic and wood.
The results of the Life Cycle Assessment provided in -Landfill, for inert material like metals (where used).
this declaration have been selected from the product -C1-C2-C3-D
with the highest environmental impact (worst-case The building deconstruction (demolition process) takes
scenario). place in the C1 module which considers energy
Depending on the application, a corresponding production and consumption in terms of diesel and all
conversion factor such as the density to convert the emissions connected with the fuel-burning process
volumetric use to mass must be taken into to run the machines. After the demolition, the product
consideration. is transported to the end-of-life processing (C2
module) where all the impacts related to the transport
The Declaration type is according to EN 15804: Cradle processes are considered. For precautionary principle
to gate with options, modules C1–C3, and module D and as a worst-case scenario, thermal treatment is the
(A1–A3, C, D) and additional modules. only end-of-life scenario considered. This is modelled
by the incineration process (module C3) where the
Declared unit product ends its life cycle.
Name Value Unit Module D accounts for potential benefits that are
Declared unit 1 kg beyond the defined system boundaries. Credits are
Gross density 0.85 - 1.8 g/cm³ generated during the incineration of wastes and related
Conversion factor to 1 kg - - electricity produced that are occurring in the A5
module.
3.3 Estimates and assumptions
3.2 System boundary For this EPD formulation and production data defined
Modules A1, A2 and A3 are taken into consideration in and collected by FEICA were considered. Production
the LCA: waste was assumed to be disposed of by incineration
- A1 Production of preliminary products without credits as a worst-case.
- A2 Transport to the plant An average of steel and plastic containers, and
- A3 Production incl. provision of energy, production of wooden pallets was considered in the LCA.
packaging as well as auxiliaries and consumables and
waste treatment 3.4 Cut-off criteria
- A4 Transport to site All raw materials submitted for the formulations and
- A5 Installation, product applied into the building production data were taken into consideration.
during A5 phase operations and packaging disposal. The manufacture of machinery, plant and other
This stage considers VOC emissions during the infrastructure required for the production of the
installation phase. The declared product does not
6 Environmental Product Declaration FEICA/EFCC/IVK/DBC – Products based on polyurethane, group 5
products under review was not taken into consideration The data quality of the background data is considered
in the LCA. to be good.
Transport of packaging materials is excluded.
3.7 Period under review
3.5 Background data Representative formulations are valid for 2021.
Data from the GaBi database SP40 (2020) was used
as background data. 3.8 Allocation
Mass allocation has been applied when primary data
3.6 Data quality have been used and implemented into the LCA model.
Representative products were applied for this EPD and
the product in the group displaying the highest 3.9 Comparability
environmental impact was selected for calculating the Basically, a comparison or an evaluation of EPD data
LCA results. The background data sets used are less is only possible if all the data sets to be compared
than 4 years old. were created according to EN 15804 and the building
Production data and packaging are based on details context, respectively the product-specific
provided by the manufacturer. The formulation used for characteristics of performance, are taken into account.
evaluation refers to a specific product.
The GaBi database SP40 (2020) was used.
4. LCA: Scenarios and additional technical information
Characteristic product properties
Information on biogenic Carbon
The packaging material contains biogenic carbon
content which is presented below.
Information on describing the biogenic Carbon
Content at factory gate
Name Value Unit
Biogenic Carbon Content in
0.297 kg C
product
Biogenic Carbon Content in
0.016 kg C
accompanying packaging
Transport to the building site (A4)
Name Value Unit
Transport distance 1000 km
Gross weight 34 - 40 t
Payload capacity 27 t
Assembly (A5)
Name Value Unit
Other resources for packaging
0.1 kg
material
Material loss 0.01 kg
Material loss regards the amount of product not used
during the application phase into the building. This
amount is 1% of the product, impacts related to the
production of this part are charged to the A5 module.
This percentage is considered as waste to disposal
and impacts of its end of life have been considered in
the LCA model and declared in A5.
End of life (C1-C3)
Name Value Unit
Collected as mixed construction
1 kg
waste
Incineration 1 kg
7 Environmental Product Declaration FEICA/EFCC/IVK/DBC – Products based on polyurethane, group 5
5. LCA: Results
DESCRIPTION OF THE SYSTEM BOUNDARY (X = INCLUDED IN LCA; ND = MODULE OR INDICATOR NOT
DECLARED; MNR = MODULE NOT RELEVANT)
BENEFITS AND
CONSTRUCTI LOADS
PRODUCT STAGE ON PROCESS USE STAGE END OF LIFE STAGE BEYOND THE
STAGE SYSTEM
BOUNDARIES
8 Environmental Product Declaration FEICA/EFCC/IVK/DBC – Products based on polyurethane, group 5
lairetam
waR
ylppus tropsnarT
gnirutcafunaM
eht
morf
tropsnarT
etis
eht
ot
etag
ylbmessA esU
ecnanetniaM
riapeR
tnemecalpeR tnemhsibrufeR
ygrene
lanoitarepO esu
retaw
lanoitarepO esu
noitcurtsnoc-eD
noitilomed tropsnarT
gnissecorp
etsaW
lasopsiD -esueR -yrevoceR -gnilcyceR laitnetop
A1 A2 A3 A4 A5 B1 B2 B3 B4 B5 B6 B7 C1 C2 C3 C4 D
X X X X X ND ND MNR MNR MNR ND ND X X X ND X
RESULTS OF THE LCA - ENVIRONMENTAL IMPACT according to EN 15804+A2: 1 kg of product based on
polyurethane, group 5
Core Indicator Unit A1-A3 A4 A5 C1 C2 C3 D
GWP-total [kg CO2-Eq.] 8.76E-1 5.27E-2 1.41E-1 2.79E-4 1.24E-2 3.30E+0 -9.50E-1
GWP-fossil [kg CO2-Eq.] 2.02E+0 5.22E-2 6.59E-2 2.66E-4 1.18E-2 2.21E+0 -9.47E-1
GWP-biogenic [kg CO2-Eq.] -1.15E+0 1.52E-4 7.50E-2 1.24E-5 5.42E-4 1.09E+0 -2.23E-3
GWP-luluc [kg CO2-Eq.] 3.70E-3 4.22E-4 4.04E-5 6.39E-9 2.79E-7 2.08E-5 -6.66E-4
ODP [kg CFC11-Eq.] 1.55E-6 6.27E-18 1.55E-8 2.84E-20 1.24E-18 2.62E-16 -9.93E-15
AP [mol H+-Eq.] 2.53E-2 1.56E-4 2.81E-4 3.60E-6 3.73E-5 1.31E-3 -1.33E-3
EP-freshwater [kg P-Eq.] 7.16E-4 1.59E-7 7.17E-6 5.75E-11 2.51E-9 4.40E-8 -1.23E-6
EP-marine [kg N-Eq.] 9.67E-3 6.96E-5 1.05E-4 1.63E-6 1.72E-5 6.31E-4 -3.43E-4
EP-terrestrial [mol N-Eq.] 9.84E-2 7.80E-4 1.10E-3 1.79E-5 1.89E-4 7.26E-3 -3.68E-3
POCP [kg NMVOC-Eq.] 6.92E-3 1.38E-4 7.17E-3 4.91E-6 3.39E-5 1.62E-3 -9.87E-4
ADPE [kg Sb-Eq.] 9.14E-6 3.74E-9 9.19E-8 8.06E-12 3.52E-10 4.65E-9 -1.56E-7
ADPF [MJ] 2.94E+1 6.94E-1 3.53E-1 3.81E-3 1.66E-1 5.87E-1 -1.61E+1
[m³ world-Eq
WDP 4.76E+1 4.66E-4 4.90E-1 5.27E-7 2.30E-5 2.17E-1 -9.86E-2
deprived]
GWP = Global warming potential; ODP = Depletion potential of the stratospheric ozone layer; AP = Acidification potential of land and water; EP =
Caption Eutrophication potential; POCP = Formation potential of tropospheric ozone photochemical oxidants; ADPE = Abiotic depletion potential for non-
fossil resources; ADPF = Abiotic depletion potential for fossil resources; WDP = Water (user) deprivation potential
RESULTS OF THE LCA - INDICATORS TO DESCRIBE RESOURCE USE according to EN 15804+A2: 1 kg of
product based on polyurethane, group 5
Indicator Unit A1-A3 A4 A5 C1 C2 C3 D
PERE [MJ] 2.06E+1 3.90E-2 9.57E-1 1.20E-5 5.25E-4 1.53E+1 -3.52E+0
PERM [MJ] 1.58E+1 0.00E+0 -5.85E-1 0.00E+0 0.00E+0 -1.45E+1 0.00E+0
PERT [MJ] 3.65E+1 3.90E-2 3.72E-1 1.20E-5 5.25E-4 8.23E-2 -3.52E+0
PENRE [MJ] 1.49E+1 6.95E-1 8.73E-1 3.81E-3 1.67E-1 1.47E+1 -1.61E+1
PENRM [MJ] 1.46E+1 0.00E+0 -5.20E-1 0.00E+0 0.00E+0 -1.41E+1 0.00E+0
PENRT [MJ] 2.95E+1 6.95E-1 3.54E-1 3.81E-3 1.67E-1 5.87E-1 -1.61E+1
SM [kg] 0.00E+0 0.00E+0 0.00E+0 0.00E+0 0.00E+0 0.00E+0 0.00E+0
RSF [MJ] 0.00E+0 0.00E+0 0.00E+0 0.00E+0 0.00E+0 0.00E+0 0.00E+0
NRSF [MJ] 0.00E+0 0.00E+0 0.00E+0 0.00E+0 0.00E+0 0.00E+0 0.00E+0
FW [m³] 1.62E+0 4.52E-5 1.65E-2 2.16E-8 9.41E-7 5.11E-3 -4.08E-3
PERE = Use of renewable primary energy excluding renewable primary energy resources used as raw materials; PERM = Use of
renewable primary energy resources used as raw materials; PERT = Total use of renewable primary energy resources; PENRE = Use of
non-renewable primary energy excluding non-renewable primary energy resources used as raw materials; PENRM = Use of non-
Caption
renewable primary energy resources used as raw materials; PENRT = Total use of non-renewable primary energy resources; SM = Use
of secondary material; RSF = Use of renewable secondary fuels; NRSF = Use of non-renewable secondary fuels; FW = Use of net fresh
water
RESULTS OF THE LCA – WASTE CATEGORIES AND OUTPUT FLOWS according to EN 15804+A2:
1 kg of product based on polyurethane, group 5
Indicator Unit A1-A3 A4 A5 C1 C2 C3 D
HWD [kg] 1.12E-5 3.23E-8 1.12E-7 3.70E-13 1.62E-11 3.34E-10 -6.41E-9
NHWD [kg] 1.36E-1 1.06E-4 4.72E-2 3.90E-7 1.70E-5 1.11E-2 -7.44E-3
RWD [kg] 6.82E-4 8.60E-7 8.73E-6 4.09E-9 1.79E-7 2.37E-5 -1.20E-3
CRU [kg] 0.00E+0 0.00E+0 0.00E+0 0.00E+0 0.00E+0 0.00E+0 0.00E+0
MFR [kg] 0.00E+0 0.00E+0 0.00E+0 0.00E+0 0.00E+0 0.00E+0 0.00E+0
MER [kg] 0.00E+0 0.00E+0 0.00E+0 0.00E+0 0.00E+0 0.00E+0 0.00E+0
EEE [MJ] 0.00E+0 0.00E+0 2.12E-1 0.00E+0 0.00E+0 0.00E+0 0.00E+0
EET [MJ] 0.00E+0 0.00E+0 3.86E-1 0.00E+0 0.00E+0 0.00E+0 0.00E+0
HWD = Hazardous waste disposed; NHWD = Non-hazardous waste disposed; RWD = Radioactive waste disposed; CRU = Components
Caption for re-use; MFR = Materials for recycling; MER = Materials for energy recovery; EEE = Exported electrical energy; EEE = Exported
thermal energy
RESULTS OF THE LCA – additional impact categories according to EN 15804+A2-optional:
1 kg of product based on polyurethane, group 5
Indicator Unit A1-A3 A4 A5 C1 C2 C3 D
[Disease
PM ND ND ND ND ND ND ND
Incidence]
[kBq U235-
IRP ND ND ND ND ND ND ND
Eq.]
ETP-fw [CTUe] ND ND ND ND ND ND ND
HTP-c [CTUh] ND ND ND ND ND ND ND
HTP-nc [CTUh] ND ND ND ND ND ND ND
SQP [-] ND ND ND ND ND ND ND
PM = Potential incidence of disease due to PM emissions; IR = Potential Human exposure efficiency relative to U235; ETP-fw = Potential
Caption comparative Toxic Unit for ecosystems; HTP-c = Potential comparative Toxic Unit for humans (cancerogenic); HTP-nc = Potential
comparative Toxic Unit for humans (not cancerogenic); SQP = Potential soil quality index
Potential Human exposure efficiency relative to U235, Disclaimer 1 – This impact category deals mainly with the
eventual impact of low dose ionizing radiation on human health of the nuclear fuel cycle. It does not consider
effects due to possible nuclear accidents, occupational exposure or radioactive waste disposal in underground
facilities. Potential ionizing radiation from the soil, radon and (from) some construction materials is also not
measured by this indicator.
ADP minerals & metals, ADP fossil, WDP, ETF-fw, HTP-c, HTP-nc, SQP, Disclaimer 2 – The results of this
environmental impact indicator shall be used with care as the uncertainties on these results are high or as there is
limited experience with the indicator.
Additional environmental impact indicators (suggested by EN15804, table 4) are not declared in the EPD. The
results of this environmental impact indicator shall be used with care as the uncertainties on these results are high
and as there is limited experience with the indicator (see ILCD classification in EN 15804, table 5). For this
reason, results based on these indicators are not considered suitable for a decision-making process and are thus
not declared in the EPD.
6. LCA: Interpretation
Due to the presence of a high content of raw materials renewable energy resources required for the
with biogenic origin, the production phase (A1-A3) is generation and supply of electricity. It should be noted
not the highest among all impact categories. The most that Primary Energy Demand – Renewable (PERT)
significant contribution to the production phase impacts generally represents a small percentage of the
is the upstream production of raw materials. Another production phase primary energy demand with the bulk
substantial contributor in the production phase, in the of the demand coming from non-renewable energy
category of Abiotic depletion potential for non-fossil resources.
resources (ADPminerals& metals), is the steel sheet Transportation to the construction site (A4) and the
used as a packaging material. Emissions associated installation process (A5) make a low contribution to all
with the manufacturing of products also have some impacts.
influence on the Formation potential of tropospheric The installation phase influences mainly the
ozone (POCP) in the production phase. In all EPDs, Photochemical ozone formation indicator, due to the
CO is the most important contributor to Global emission of VOC during the operations. These
2
Warming Potential (GWP). For the Acidification emissions are not directly related to the pre-products in
Potential (AP), NOx and SO contribute the largest the resins, but they are related to the reaction products
2
share. In some cases, HCl in water also impacts AP between pre-products and air components (water and
due to the use of TiO .as a pigment. oxygen).
2
The majority of life cycle energy consumption takes The end-of-life phases has a significantly influence on
place during the production phase (A1-A3). Significant climate change indicators, due to the incineration
contributions to Primary Energy Demand – Non- processes occurring in the C3 module, the process
renewable (PENRT) come from the energy resources used for modelling the thermal treatment process of
used in the production of raw materials. The largest the resin.
contributor to Primary Energy Demand – Renewable
(PERT) impacts comes from the consumption of
7. Requisite evidence
VOC - either an attestation of compliance with,
Special tests and evidence have not been carried out - or documentation of test data that are required in
or provided within the framework of drawing up this any of the existing regulations or in any of the existing
Model EPD. Some member states require special voluntary labelling programs for low-emitting products,
documentation on VOC emissions into indoor air for as far as these
specific areas of application. This documentation, as (1) include limits for the parameters TVOC, TSVOC,
well as documentation for voluntary VOC labelling, has carcinogens, formaldehyde, acetaldehyde, LCI limits
to be provided separately and is specific for product in for individual substances (including but not limited to
question. the European list of harmonized LCIs), and the R
value;
Evidence pertaining to VOC emissions shall show (2) base their test methods on EN 16516;
9 Environmental Product Declaration FEICA/EFCC/IVK/DBC – Products based on polyurethane, group 5
(3) perform testing and apply the limits after 28 days - TVOC: 1000 µg/m³
of storage in a ventilated test chamber, under the - TSVOC: 100 µg/m³
conditions specified in EN 16516; some regulations - Each carcinogen: 1 µg/m³
and programs also have limits after 3 days, on top of - Formaldehyde: 100 µg/m³
the 28 days limits; - LCI: different per substance involved
(4) express the test results as air concentrations in - R value: 1 (meaning that, in total, 100 % of the
the European Reference Room, as specified in EN combined LCI values must not be exceeded).
16516. Informative Annexes (2 tables):
Table 1 shown below is an overview of the most
Examples of such regulations are the Belgian Royal relevant regulations and specifications as of October
Decree C-2014/24239, or the German AgBB/ ABG. 2021, as regards requirements after 3 days of storage
Examples of such voluntary labelling programs are in a ventilated test chamber.
EMICODE, Blue Angel or Indoor Air Comfort. Table 2 provides an overview of the most relevant
regulations and specifications as of October 2021, as
Relevant test results shall be produced either by an regards requirements after 28 days of storage in a
ISO 17025 accredited commercial test lab or by a ventilated test chamber. Some details may be missing
qualified internal test lab of the manufacturer. in the table due to lack of space. Values given
Examples for the applied limits after 28 days of storage represent maximum values/limits.
in a ventilated test chamber are:
8. References
10 Environmental Product Declaration FEICA/EFCC/IVK/DBC – Products based on polyurethane, group 5
ETAG 033 ISO 3219-2:2021, Rheology - Part 2: General
Liquid applied bridge deck waterproofing kits principles of rotational and oscillatory rheometry
ISO 48-4 EN ISO 7783
ISO 48-4:2018, Rubber, vulcanized or thermoplastic - EN ISO 7783:2019-02, Paints and varnishes -
Determination of hardness- Part 4: Indentation Determination of water-vapour transmission properties
hardness by durometer method (Shore hardness) - Cup method
EN ISO 717-1 EN 12004
EN ISO 717-1:2020 Acoustics - Rating of sound EN12004:2012, Adhesives for ceramic tiles
insulation in buildings and of building elements -
Part 1: Airborne sound insulation EN 12004-1
EN 12004-1:2017, Adhesives for ceramic tiles – Part 1:
EN 1062-3 Requirements, assessment and verification of
EN 1062-3:2008-04, Paints and varnishes - Coating constancy of performance, classification and marking
materials and coating systems for exterior masonry
and concrete - Part 3: Determination of liquid water EN 12004-2
permeability EN 12004-2:2017, Adhesives for ceramic tiles - Part 2:
Test methods
EN 1062-6
EN 1062-6:2002-10, Paints and varnishes - Coating EN 13501-1
materials and coating systems for exterior masonry EN 13501-1:2018, Fire classification of construction
and concrete - Part 6: Determination of carbon dioxide products and building elements - Part 1: Classification
permeability using data from reaction to fire tests
EN 1279-4 EN 13813
EN 1279-4:2002 Glass in building - Insulating glass EN 13813:2002-10, Screed material and floor screeds
units - Part 4: Methods of test for the physical - Screed materials - Properties and requirements
attributes of edge seals
EN 13892-8
EN 1504-2 EN 13892:2003-02, Methods of test for screed
EN 1504-2:2004-12, Products and systems for the materials - Part 8: Determination of bond strength
protection and repair of concrete structures -
Definitions, requirements, quality control and ISO 14025
evaluation of conformity - Part 2: Surface protection DIN EN ISO 14025:2011-10, Environmental labels and
systems for concrete declarations — Type III environmental declarations —
Principles and procedures
EN 1504-4
EN 1504-4:2004-11, Products and systems for the EN 14891
protection and repair of concrete structures - EN 14891:2012-04, Liquid applied water impermeable
Definitions, requirements, quality control and products for use beneath ceramic tiling - Definitions,
evaluation of conformity- Part 4: Structural bonding specifications and test methods
EN 1504-5 EN 15804
EN 1504-5:2004-12, Products and systems for the EN 15804:2019+A2, Sustainability of construction
protection and repair of concrete structures - works — Environmental Product Declarations — Core
Definitions, requirements, quality control and rules for the product category of construction products
evaluation of conformity - Part 5: Concrete injection
EN 16516
EN 1542 EN 16516:2017
EN 1542:1999-07, Products and systems for the Construction products - Assessment of release of
protection and repair of concrete structures - Test dangerous substances - Determination of emissions
methods - Measurement of bond strength by pull-off into indoor air
EN 1771 EN ISO 17025
EN 1771:2004-11, Products and systems for the EN ISO 17025:2018-03
protection and repair of concrete structures - Test General requirements for the competence of testing
methods - Determination of injectability and splitting and calibration laboratories
test
EN ISO 17178
ISO 2811-1 EN ISO 17178:2020-06, Adhesives - Adhesives for
ISO 2811-1:2016, Paints and varnishes - bonding parquet to subfloor - Test methods and
Determination of density - Part 1: Pycnometer method minimum requirements
EN ISO 3219 EN 17333-2
EN ISO 3219:1994-10, Plastics - Polymers/resins in EN 17333-2:2020+AC:2020, Characterisation of one
the liquid state or as emulsions or dispersions - component foam - Part 2: Expansion characteristics
Determination of viscosity using a rotational viscometer
with defined shear rate EN 17333-3
EN 17333-3:2020, Characterisation of one component
ISO 3219-2 foam - Part 3: Application
11 Environmental Product Declaration FEICA/EFCC/IVK/DBC – Products based on polyurethane, group 5
GaBi 10 software & documentation
EN 17333-4 Data base for Life Cycle Engineering LBP, University
EN 17333-4:2020, Characterisation of one component of Stuttgart and Sphera, documentation of GaBi 10
foam - Part 4: Mechanical strength data sets http://documentation.gabi-software.com/,
2020
EN 17333-5
EN 17333-5:2020, Characterisation of one component German AgBB
foam - Part 5: Insulation Committee for Health-related Evaluation of Building
Products: health-related evaluation of emissions of
EN ISO 22636 volatile organic compounds (VOC and SVOC) from
EN ISO 22636:2020, Adhesives - Adhesives for floor building products; status: June 2012
coverings - Requirements for mechanical and electrical www.umweltbundesamt.de/produkte/bauprodukte/agb
performance b.htm
EAD 030350-00-0402 IBU 2021
EAD 030350-00-0402:2018-08, Liquid Applied Roof Institut Bauen und Umwelt e.V.: General Instructions
Waterproofing Kits for the EPD programme of Institut Bauen und Umwelt
e.V. EPD programme. Version 2.0. Berlin: Institut
EAD 030352-00-0503 Bauen und Umwelt e.V., 2021
EAD 030352-00-0503:2019-01, Liquid applied www.ibu-epd.com
watertight covering kits for wet room floors and/or walls
ift-Guideline VE-08/4
2000/532/EC ift-Guideline VE-08/4:2017, Beurteilungsgrundlage für
Commission decision dated 3 May 2000 replacing geklebte Verglasungssysteme
decision 94/3/EC on a waste directory in accordance
with Article 1 a) of Council Directive 75/442/EEC on Indoor Air Comfort
waste and Council decision 94/904/EC on a directory Product certification by Eurofins, Hamburg, Germany
of hazardous waste in terms of Article 1, paragraph 4 www.eurofins.com
of Directive 91/689/EEC on hazardous waste
PCR Part A
Belgian Royal Decree C-2014/24239 Product Category Rules for Building-Related Products
Belgisch Staatsblad 8 MEI 2014, p. 60603. — and Services, Part A: Calculation Rules for the Life
Koninklijk besluit tot vaststelling van de Cycle Assessment and Requirements on the Project
drempelniveaus voor de emissies naar het report, Version 1.1, Institut Bauen und Umwelt e.V.,
binnenmilieu van bouwproducten voor bepaalde 2021-01
geoogde gebruiken
PCR Part B
Blue Angel Product Category Rules for Construction Products,
Environmental label organised by the federal Part B: Reaction resin products, Institut Bauen und
government of Germany www.blauer-engel.de Umwelt e.V., 2019-01
CPR RAL-GZ 716
CPR Regulation (EU) No 305/2011 of the European RAL-GZ 716:2019-04 part 2, Kunststoff-
Parliament and of the Council of 9 March 2011 laying Fensterprofilsysteme - Gütesicherung
down harmonised conditions for the marketing of
construction products and repealing Council Directive REACH
89/106/EEC Directive (EG) No. 1907/2006 of the European
Parliament and of the Council dated 18 December
Decopaint Directive 2006 on the registration, evaluation, approval and
Directive 2004/42/CE of the European Parliament and restriction of chemical substances (REACH), for
the council of 21 April 2004 on the limitation of establishing a European Agency for chemical
emissions of volatile organic compounds due to the substances, for amending Directive 1999/45/EC and
use of organic solvents in certain paints and varnishes for annulment of Directive (EEC) No. 793/93 of the
and vehicle refinishing products and amending Council, Directive (EC) No. 1488/94 of the
Directive 1999/13/EC Commission, Guideline 76/769/EEC of the Council and
Guidelines 91/155/EEC, 93/67/EEC, 93/105/EC and
EMICODE 2000/21/EC of the Commission.
EMICODE, GEV – Gemeinschaft
Emissionskontrollierte Verlegewerkstoffe, Klebstoffe
und Bauprodukte e. V. (pub.).www.emicode.de
12 Environmental Product Declaration FEICA/EFCC/IVK/DBC – Products based on polyurethane, group 5
Publisher
Institut Bauen und Umwelt e.V. Tel +49 (0)30 3087748- 0
Hegelplatz 1 Fax +49 (0)30 3087748- 29
10117 Berlin Mail info@ibu-epd.com
Germany Web www.ibu-epd.com
Programme holder
Institut Bauen und Umwelt e.V. Tel +49 (0)30 - 3087748- 0
Hegelplatz 1 Fax +49 (0)30 – 3087748 - 29
10117 Berlin Mail info@ibu-epd.com
Germany Web www.ibu-epd.com
Author of the Life Cycle
Assessment Tel +49 711 341817-0
Sphera Solutions GmbH Fax +49 711 341817-25
Hauptstraße 111- 113 Mail info@sphera.com
70771 Leinfelden-Echterdingen Web www.sphera.com
Germany
Owner of the Declaration
EFCC - European Federation for Tel +32289720-39
Construction Chemicals Fax +32289720-37
Boulevard du Triomphe 172 Mail info@efcc.be
1160 Brussels Web www.efcc.eu
Belgium
Tel +32 (0)267 673 20
FEICA - Association of the Fax +32 (0)267 673 99
European Adhesive and Sealant Mail info@feica.eu
Industry Web www.feica.eu
Avenue E. van Nieuwenhuyse 2
B-1160 Brussels
Belgium
Tel +49 (0)69 2556-1318
Fax +49 (0)69 2556-1319
Mail info@deutsche-bauchemie.de
Deutsche Bauchemie e.V. Web www.deutsche-bauchemie.de
Mainzer Landstr. 55
60329 Frankfurt
Germany
Tel +49 (0)211 67931-10
Fax +49 (0)211 67931-33
Mail info@klebstoffe.com
Industrieverband Klebstoffe e.V Web www.klebstoffe.com
Völklinger Straße 4
40219 Düsseldorf
Germany
