ENVIRONMENTAL PRODUCT DECLARATION
as per ISO 14025 and EN 15804+A2
Owner of the Declaration Hansgrohe Group
Publisher Institut Bauen und Umwelt e.V. (IBU)
Programme holder Institut Bauen und Umwelt e.V. (IBU)
Declaration number EPD-HAN-20230020-ICC2-EN
Issue date 24.02.2023
Valid to 23.02.2028
Overhead Showers
Hansgrohe Group
www.ibu-epd.com | https://epd-online.com
1. General Information
Hansgrohe Group Overhead Showers
Programme holder Owner of the declaration
IBU – Institut Bauen und Umwelt e.V. Hansgrohe Group
Hegelplatz 1 Auestr. 5-9
10117 Berlin 77761 Schiltach
Germany Germany
Declaration number Declared product / declared unit
EPD-HAN-20230020-ICC2-EN One (1)
piece of an average overhead shower incl. packaging
This declaration is based on the product category rules: Scope:
Fittings and showers, 01.08.2021 This average EPD was determined on the basis of a weighted average of
(PCR checked and approved by the SVR) production volume from 2020 and relates to the plants in Wasselonne,
France, Offenburg and Schiltach, Germany, Shanghai, China and
Alpharetta, USA. This average EPD is valid for the whole product group of
Issue date chrome plated overhead showers. The EPD was formed from >97% of the
products involved in the sales quantity.
24.02.2023
The owner of the declaration shall be liable for the underlying information
and evidence; the IBU shall not be liable with respect to manufacturer
information, life cycle assessment data and evidences.
Valid to
23.02.2028 The EPD was created according to the specifications of EN 15804+A2. In
the following, the standard will be simplified as EN 15804.
Verification
The standard EN 15804 serves as the core PCR
Independent verification of the declaration and data according to ISO
14025:2011
internally X externally
Dipl.-Ing. Hans Peters
(Chairman of Institut Bauen und Umwelt e.V.)
Florian Pronold Dr Naeem Adibi,
(Managing Director Institut Bauen und Umwelt e.V.) (Independent verifier)
1 Environmental Product Declaration - Hansgrohe Group - Overhead Showers
2. Product
The overhead showers are delivered singularly packaged. The
2.1 Product description/Product definition packaging is
Overhead showers customized to the size of the product and supplies. Customers
essentially comprise of a housing made of plastic materials or can order single
metal and a jet products or multiple products with outer packaging.The
disc as well as several assembly parts of various materials. The products with the smallest and the largest volume have
shower surface dimensions between 110x80x130 mm and 585x145x795 mm.
is usually chrome-plated by means of various galvanic process
stages. 2.5 Base materials/Ancillary materials
The material composition (incl. packaging) of an average
For the use overhead shower is as follows:
and application of the product the respective national provisions Name Value Unit
at the place
Cardboard, Paper 29.4 %
of use apply, in Germany for example the building codes of the
Brass 25.2 %
federal states
and the corresponding national specifications. Other plastics 14.1 %
Polyphenylene 13.1 %
The products comply with Stainless steel 8.6 %
the applicable standards and regulations listed below. Following
Acrylonitrile butadiene styrene 7.8 %
standards apply to all hand showers and head showers to
Zinc 1.3 %
prove product safety:
Other metals 0.2 %
• EN 1112:2008: Sanitary tapware – Shower outlets for
Other material 0.2 %
sanitary tapware for water supply systems of type 1 and
type 2 Aluminium 0.1 %
• ISO 3822: Acoustics – Laboratory tests on noise The parts which are made of brass contain between 0.2 and
emission from appliances and equipment used in water 1.4% lead.
supply installations
This product contains substances listed in the candidate list
2.2 Application
(date: 17.12.2021) exceeding 0.1 percentage by mass: Lead
Overhead showers are showers that are fixed installed more
(CAS number 7439-92-1) as a component of the brass alloy
than man-high. They can be
has been on the candidate list of the Reach Regulation
installed on the wall or on/in the ceiling. Some overhead
(Regulation (EC) No. 1907/2006) since 27.06.2018.
showers have two or
three spray types to choose between, some only have one.
This product/article/at least one partial article contains other
They are used for
CMR substances in categories 1A or 1B which are not on the
showering.
candidate list, exceeding 0.1 percentage by mass: no.
2.3 Technical Data
Biocide products were added to this construction product or it
The technical specifications of the products within the scope of
has been treated with biocide products (this then concerns a
the EPD shall be listed, including the reference to the test
treated product as defined by the (EU) Ordinance on Biocide
methods/test standards for each specification.
Products No. 528/2012): no.
For products with CE marking, the technical specifications must 2.6 Manufacture
be specified in accordance with information in the declaration of
performance. The properties relevant to the product should be
specified in the table below. If no information is given for
properties, an explanation must be given in the background
report to the EPD as to why the property is not relevant to the
product.
Constructional data
Name Value Unit
Maximum load temperature
42 °C
permanent operation
Maximum load temperature
70 °C
temporary operation
Flow rate (indications for Depending on flow rate m3/h No. 1: The
pressure range of 1-3 bar) class 0,54 to 2,28 plastic jet body is injected.
Sound emissions <30 dB No. 2: The
plastic upper part of housing is injected.
Performance data of the product with respect to its
characteristics in accordance with the relevant technical
provision (no
CE-marking).
No. 3: The
2.4 Delivery status upper part of housing is galvanized.
2 Environmental Product Declaration - Hansgrohe Group - Overhead Showers
All packaged products fit on a reusable euro
No. 4: The pallet.
plastic thread nipple is injected.
2.10 Condition of use
To protect
the overhead showers and make them durable, the product is
No. 5: All usually
the parts are assembled and packed. chrome-plated. Nevertheless, there are no unhealthy
contaminants in the water.
To ensure the longevity of the product, it should be used and
cleaned
Any production waste generated is disposed accordingly. In regularly.
individual cases, the production may differ slightly from the
2.11 Environment and health during use
procedure.
Our products do not emission any contaminants or substances
2.7 Environment and health during manufacturing that are
Hansgrohe SE tries to keep the harmful to the environment or health during the use phase.
impact on people and the environment as low as possible when
2.12 Reference service life
manufacturing its
products. The quality and durability of our overhead showers is designed
Hazards at workplaces are regularly for a
assessed and reduced to a minimum. product life of about 20 years. Which on average is
approximately the duration
of use by the consumers. With few
exceptions, all products have a five-year warranty. Furthermore,
For example, in basic production, an after-sale
sawing or grinding work is mainly carried out by robots, and in service warranty of 15 years is provided.
electroplating,
2.13 Extraordinary effects
chemicals are dosed automatically via appropriate pump
Fire
stations.
The products are not classified as
building materials (building products) and are not subject to DIN
4102 and EN
13501-1.
Emissions that are hazardous to
health are extracted directly at the source and cleaned by filter Fire protection
systems. Name Value
Building material class
Burning droplets
Workplace and emission limits are Smoke gas development
regularly monitored and are far below the prescribed limits.
Water
If a room in which the products offered by Hansgrohe are
installed is flooded with water, the products are not affected in
To reduce environmental impact, their function.
water and production waste are recycled wherever possible. There will be no environmental impact.
In addition, all production sites are certified according to the
DIN EN Mechanical destruction
ISO standards 14001 (environment), 50001 (energy), 45001 (occupationIfa tlhe surface of the coating is destroyed by a mechanical
health and safety) and 9001 (quality). Continuous improvement stress, there is a possibility of corrosion.
of environmental and occupational safety performance is thus In the event of mechanical damage, the products may need to
guaranteed. be replaced due to possible sharp cut edges.
2.8 Product processing/Installation 2.14 Re-use phase
The overhead showers are screwed on by hand (tools: none). The overhead showers are not taken back by the manufacturer
for the
2.9 Packaging
purpose of reuse. Users can disassemble the products
For product protection the overhead showers are individually
repeatedly within the
packed in a
reference utilization period and reuse it elsewhere.
cardboard box, which consists of approximately 80% recycled
material. The 2.15 Disposal
cardboard is always printed with lead-free ink and in some The waste code of the product is AVV 20 03 01. Disassembly of
cases additionally the products consists of the same steps as assembly, in
coated with clear topcoat. The inlay of the packaging consists reverse order.
of folded All metal components can be recycled (as
cardboard, fiber form or plastic bags, depending on the product. scrap).
The packaging can be fully recycled.
3 Environmental Product Declaration - Hansgrohe Group - Overhead Showers
substance recycling is established, disposal takes place via the
All plastic components have a high calorific waste
value and can be sent for thermal recycling. incineration plant.
2.16 Further information
Additional information about our products can be found at
In countries where no thermal recycling or https://www.hansgrohe.com.
3. LCA: Calculation rules
for the products and considered as zero.
3.1 Declared Unit
The results of this EPD are valid for the following functional Module B2:
unit:
Provide sanitary function for one (1) average overhead shower
unit used in accordance with the manufacturer's Maintenance
recommendations for a 20-year life, following the expenses are declared in this module and consist of weekly
manufacturer's operating instructions. An average conditioned cleaning expenses
overhead shower is considered the baseline flow. for this product.
Weighted averaging based on production tonnages in 2020 is
chosen as basis for creating the environmental profile. 179
different overhead showers were considered. Module
Functional unit B6:
Name Value Unit
This
Declared unit 1 pce.
module considers the energy input required to bring water to a
Functional unit 1 pce. certain
Functional unit with packaging 2.31 kg temperature for the use of a gas low temperature boiler
Packaging 0.64 kg (scenario B6/1) and for the use of an electric instantaneous
water heater (scenario B6/2).
Weight range of the products examined 0.26 - 13.59 kg
Other declared units are allowed if the conversion is shown
transparently. Module
B7:
For IBU core EPDs (where clause 3.6 is part of the EPD): for
average EPDs, an estimate of the robustness of the LCA
values must be made, e.g. concerning the variability of the This
production process, geographical representativeness and the module considers the water consumption that can be expected
influence of background data and preliminary products depending on the
compared to the environmental impacts caused by the actual function of the product family.
production.
Modules C1-C4:
The modules include the environmental impacts for dismantling
3.2 System boundary
of the products and the treatment of the waste fractions until
This representative EPD follows the EPD type "cradle to gate -
the end-of-waste status (EoW) is reached, including the
with options". The following life cycle modules are declared:
associated transports at the end of the product life cycle.
Modules A1-A3:
Module D:
The product stage begins with considering the production of the
necessary raw materials and energies, including all
corresponding upstream chains and the actual procurement
transports. Furthermore, the entire manufacturing phase was
Identification
mapped, including the treatment of production waste until the
of the benefits and costs of the product outside the system
end-of-waste status (EoW) was reached. Green electricity from
boundary. For waste,
hydropower is used for the manufacturing processes in
paper and plastics, these consist of energy credits from thermal
Germany. Green electricity from hydropower and wind power
utilization (A3,
(50% each) is used for the French production site. US electricity
A5 and C3) in the form of the average European electricity mix
mix is used for the US production site. Chinese electricity mix is
or thermal energy
used for the Chinese production site, although electricity from
from natural gas. Recycling of paper, plastic and metal scrap
photovoltaic is partly used there.
results in
credits of the respective raw materials for the primary material
Module A4:
portion of the input. The loads of the waste incineration and
All distribution transports to the customers were considered.
recycling processes are assigned to the respective modules
Module A5:
(A3, A5 and C3) and
This module covers the installation process with the
not to module D.
corresponding packaging waste generated that needs to be
disposed. 3.3 Estimates and assumptions
Energy and water consumption, material amount for coating as
Modules B1 & B3-B5: well as waste during production could only be determined on
These modules were considered, but evaluated as not relevant concrete, existing products and not on the average product.
4 Environmental Product Declaration - Hansgrohe Group - Overhead Showers
The highest value of all inputs and outputs for energy, waste cycle assessment data were collected in 2020.
and coating of the top seller, the lightest and the heaviest
product was used for the calculation of energy, water, waste 3.8 Geographic Representativeness
and coating. For the incineration with energy recovery (thermal Land or region, in which the declared product system is
and electric) of waste, an r1 value of > 0.6 is assumed. The net manufactured, used or handled at the end of the product´s
efficiency for the average waste incinerated is between 38 % lifespan: Global
and 44 %, depending on the type of waste respectively the
disposal data set.
3.9 Allocation
3.4 Cut-off criteria For the production process nearly all raw materials, precursors
The and supplies could be assigned to the declared product.
effect associated with the neglected mass shares is less than Energy, water, galvanization process and production waste
5% of the were assigned to the highest value of either the heaviest,
effect categories per module. The minimum limit of 1% total lightest or most sold product of the product group. No
mass and the use byproducts are produced and no allocation is required.
of renewable and nonrenewable primary energy is not Some of the brass losses from brass processing in module A3
exceeded. are directly reused by Hansgrohe and are modelled as a closed
loop. Another part of the brass losses (brass particles and
3.5 Background data dusts) is disposed of as waste (without debits and credits).
The LCA software GaBi 10.6 was used to model the life cycle. Credits for plastics, paper and cardboard recycled in A5 and
The entire manufacturing process, as well as energy metallurgical waste in C3 are credited in module D.
consumption, were modelled on the basis of manufacturer Credits for the energy recovery of incinerated production waste
specific data. in A1-3, paper, cardboard and plastics in A5 and plastics and
However, generic background datasets were used for the other materials in C3 are credited in module D.
upstream and downstream processes. The majority of the The loads for waste water treatment and waste disposal of core
background datasets used were taken from the current version sand, waste oil and hazardous waste from the manufacturing
(2021.2) of the GaBi database. Ecoinvent Version 3.6 (2019) phase are allocated to module A3.
datasets were only used when suitable GaBi datasets were not Packaging:
available. For paper and cardboard, recycling (91 %) and energy recovery
(9 %) are considered on a pro rata basis. For plastic, a
3.6 Data quality proportionate recycling (52 %), energy recovery (48 %)
The background datasets used for accounting purposes mainly considered, based on Eurostat.
originate from the respective updated GaBi databases at the Deconstructed product at the end of life:
time of calculation. The data for the examined products was Since the product has a high plastic content, it is assumed that
captured on 95% of the plastic and metal components are incinerated (C3)
the basis of evaluations of internal production and and 5% are disposed in landfill (C4). The metal components are
environmental data, the collection of LCA relevant data within incinerated without energy recovery and the plastic
the supply chain, as well as the evaluation of relevant data for components are incinerated with energy recovery.
the energy supply. The collected
data were checked for plausibility and consistency. Good 3.10 Comparability
representativity can be assumed. Basically, a comparison or an evaluation of EPD data is only
possible if all the data sets to be compared were created
For the assessment of the variability of the results, all products according to EN 15804 and the building context, respectively
were balanced in addition to the average product. See at the product-specific characteristics of performance, are taken
chapter 6 for explanation of the variability. into account.
The used background database has to be mentioned.
3.7 Period under review
Life
4. LCA: Scenarios and additional technical information
Name ValueUnit
Characteristic product properties of biogenic carbon
Biogenic carbon content in accompanying kg
The biogenic carbon content quantifies the amount of biogenic 0.26
packaging C
carbon in a construction product leaving the factory gate, and it
shall be separately declared for the product and for any Note: 1 kg of biogenic carbon is equivalent to 44/12 kg of CO 2.
accompanying packaging.
If the total mass of biogenic carbon containing materials is less
than 5 % of the total mass of the product and accompanying The following technical information is a basis for the declared
packaging, the declaration of biogenic carbon content may be modules.
omitted. The mass of packaging containing biogenic carbon
Transport to the building site (A4)
shall always be declared.
Name ValueUnit
Transport distance (Truck) 630 km
Information on describing the biogenic Carbon Content at
factory gate Capacity utilisation (including empty runs) (Truck) 55 %
The biogenic carbon content was calculated based on the Transport distance (Container Ship) 4349 km
factors from the Capacity utilisation (Container Ship) 80 %
Thünen Intitute.
Installation into the building (A5)
5 Environmental Product Declaration - Hansgrohe Group - Overhead Showers
No Hansgrohe
additional resources or energy are required for the installation. SE declares a Service Life of 20 years as an empirical value for
The packaging is disposed the overhead showers when used in accordance with the care
either by recycling or incineration. instructions. This
Name Value Unit
value is
Packaging (Paper, cardboard and plastic) 0.635 kg
based on their technical service centre's statistics on service
Maintenance (B2) life in
the
For
market and complaints.
module B2, it is assumed that a weekly cleaning of the product
takes place, Name Value Unit
with 0.5 liter of water containing 1.5% soap. Life Span according to the manufacturer 20 a
Name Value Unit
Operational energy use (B6) and Operational water use
Maintenance cycle (cleaning) 1040 Number/RSL
(B7)
Water consumption/Cycle weekly
0.5 Liter/cycle Name Value Unit
(cleaning)
Water consumption 96.3 m3
Soap concentration (cleaning) 1.5 %
Energy demand 4480 kWh
Water consumption (cleaning) 0.52 m3
Auxiliary Soap/Tensides (cleaning) 7.8 kg End of life (C1-C4)
Name Value Unit
In case a reference service life according to applicable ISO Collected as mixed construction waste 1.676 kg
standards is declared then the assumptions and in-use Energy recovery 1.593 kg
conditions underlying the determined RSL shall be declared. In
Landfilling 0.084 kg
addition, it shall be stated that the RSL applies to the reference
conditions only.
Reuse, recovery and/or recycling potentials (D), relevant
The same holds for a service life declared by the manufacturer. scenario information
Corresponding information related to in-use conditions needs The
not be provided if a service life taken from the list of service life energy generated from energy recovery as well as recycled
by BNB is declared. materials are
assigned to module D as possible potentials or avoided loads in
subsequent systems. Credits are only given for the primary
Service life
portion of
the inputs.
6 Environmental Product Declaration - Hansgrohe Group - Overhead Showers
5. LCA: Results
The following table shows the result of the LCA for 1 piece of an average overhead shower. The results in the B-module are based on a
lifetime of 20 years. Scenario B6/1
shows the result for the use of a gas low temperature boiler. Scenario B6/2
shows the result for the use of an electric instantaneous water heater.
DESCRIPTION OF THE SYSTEM BOUNDARY (X = INCLUDED IN LCA; MND = MODULE OR INDICATOR NOT DECLARED; MNR
= MODULE NOT RELEVANT)
Benefits and
Construction loads beyond
Product stage Use stage End of life stage
process stage the system
boundaries
la ire ta m w a Ry lp p u s tro p s n a rT g n iru tc a fu n a M e h t m o rf tro p s n a rTe tis e h t o t e ta g y lb m e s s A e s U e c n a n e tn ia M ria p e R tn e m e c a lp e R tn e m h s ib ru fe R y g re n e la n o ita re p Oe s u re ta w la n o ita re p Oe s u n o itc u rts n o c -e Dn o itilo m e d tro p s n a rT g n is s e c o rp e ts a W la s o p s iD -e s u e R-y re v o c e R-g n ilc y c e Rla itn e to p
A1 A2 A3 A4 A5 B1 B2 B3 B4 B5 B6 B7 C1 C2 C3 C4 D
X X X X X X X X X X X X X X X X X
RESULTS OF THE LCA - ENVIRONMENTAL IMPACT according to EN 15804+A2: 1 piece average overhead shower incl.
packaging
Parameter Unit A1-A3 A4 A5 B1 B2 B3 B4 B5 B6/1 B6/2 B7 C1 C2 C3 C4 D
GWP-total kg CO 2 4.45E 2.09E- 9.79E- 0 2.56E 0 0 0 1.2E+03 1.78E 5.7E+01 0 2.85E- 1.33E 4.63E-03 -1.8E+00
eq +00 01 01 +01 +03 02 +00
GWP-fossil kg CO 2 5.38E 2.08E- 4.17E- 0 1.96E 0 0 0 1.2E+03 1.78E 5.7E+01 0 2.83E- 1.33E 4.63E-03 -8.73E-
eq +00 01 02 +01 +03 02 +00 01
GWP- kg CO 2 -9.37E- 0 9.37E- 0 0 0 0 0 0 0 0 0 0 0 0 -9.26E-
biogenic eq 01 01 01
GWP-luluc kg CO 2 8.31E-03 1.01E- 1.18E- 0 6.02E 0 0 0 6.06E- 2.52E 4.61E- 0 2.32E- 1.11E-044.39E-06 -1.22E-
eq 03 04 +00 02 +00 02 04 03
kg CFC11 3.31E- 3.96E- 1.09E- 4.31E- 5.39E- 5.61E- 3.76E- -1.59E-
ODP 3.91E-09 0 0 0 0 4.26E-11 0 1.11E-17
eq 17 16 06 13 13 18 10 09
3.31E- 5.96E- 6.64E- 7.34E- 3.71E 4.75E- 3.76E- -1.03E-
AP mol H+ eq 2.91E-02 0 0 0 0 1.4E-01 0 1.45E-05
03 05 02 01 +00 05 04 03
EP- 3.87E- 9.87E- 5.81E- 1.09E- 4.78E- 6.07E- 8.44E- 1.69E- -5.52E-
kg P eq 3.02E-05 0 0 0 0 0 3.69E-07
freshwater 07 08 04 04 03 02 08 07 06
9.02E- 1.51E- 3.12E- 2.66E- 1.87E- 1.37E- -3.59E-
EP-marine kg N eq 4.23E-03 2.11E-05 0 0 0 0 8.8E-01 0 3.5E-06
04 02 01 01 05 04 04
9.92E- 2.47E- 1.81E- 3.41E 9.24E 2.14E- 1.75E-
EP-terrestrial mol N eq 4.46E-02 0 0 0 0 4.2E-01 0 3.83E-05 -3.8E-03
03 04 01 +00 +00 04 03
kg
2.48E- 5.24E- 6.04E- 2.39E 1.08E- 4.24E- 3.66E- -9.49E-
POCP NMVOC 1.3E-02 0 0 0 0 9.1E-01 0 1.11E-05
03 05 02 +00 01 05 04 04
eq
1.35E- 5.77E- 6.43E- 5.24E- 7.43E- 2.52E- 1.62E- -7.61E-
ADPE kg Sb eq 8.55E-04 0 2.11E-05 0 0 0 0 3.2E-10
08 09 05 04 06 09 08 07
9.71E 2.67E 3.31E- 4.52E 2.05E 3.17E 5.87E 3.78E- 9.07E- -1.33E
ADPF MJ 0 0 0 0 0 6.73E-02
+01 +00 01 +02 +04 +04 +02 01 01 +01
m3 world
1.78E 1.28E- 1.19E- 6.93E 3.14E 2.86E 1.76E 2.64E- 1.46E- -4.99E- -5.64E-
WDP eq 0 0 0 0 0
+00 03 02 +00 +00 +02 +01 04 01 05 02
deprived
GWP = Global warming potential; ODP = Depletion potential of the stratospheric ozone layer; AP = Acidification potential of land and water; EP =
Eutrophication potential; POCP = Formation potential of tropospheric ozone photochemical oxidants; ADPE = Abiotic depletion potential for non-fossil
resources; ADPF = Abiotic depletion potential for fossil resources; WDP = Water (user) deprivation potential)
RESULTS OF THE LCA - INDICATORS TO DESCRIBE RESOURCE USE according to EN 15804+A2: 1 piece average overhead
shower incl. packaging
Parameter Unit A1-A3 A4 A5 B1 B2 B3 B4 B5 B6/1 B6/2 B7 C1 C2 C3 C4 D
1.87E 9.36E 1.46E 1.73E -4.76E
PERE MJ 9.85E-021.05E+01 0 0 0 0 1.8E+02 0 2.18E-023.24E-01 4.91E-03
+01 +01 +04 +02 +00
1.03E -1.03E
PERM MJ 0 0 0 0 0 0 -1E+00 0 0 0 0 0 0 0
+01 +01
9.36E 1.79E 1.46E 1.73E -4.76E
PERT MJ 2.9E+01 9.85E-02 1.08E-01 0 0 0 0 0 2.18E-023.24E-01 4.91E-03
+01 +02 +04 +02 +00
8.22E 2.68E 4.52E 2.05E 3.17E 5.87E 1.47E -1.33E
PENRE MJ 8.07E-01 0 0 0 0 0 3.8E-01 7.95E-01
+01 +00 +02 +04 +04 +02 +01 +01
-4.75E- -1.38E -7.27E-
PENRM MJ 1.5E+01 0 0 0 0 0 0 -1E+00 0 0 0 0 0
01 +01 01
9.72E 2.68E 4.52E 2.05E 3.17E 5.87E -1.33E
PENRT MJ 3.32E-01 0 0 0 0 0 3.8E-01 9.07E-01 6.73E-02
+01 +00 +02 +04 +04 +02 +01
7 Environmental Product Declaration - Hansgrohe Group - Overhead Showers
1.38E
SM kg 0 0 0 0 0 0 0 0 0 0 0 0 0 0 7.88E-02
+00
RSF MJ 4.94E-24 0 0 0 0 0 0 0 0 0 0 0 0 0 0 0
NRSF MJ 0 0 0 0 0 0 0 0 0 0 0 0 0 0 0 0
1.42E -2.95E-
FW m3 5.88E-021.14E-04 3.28E-04 0 1.62E-01 0 0 0 2E-01 5.01E-01 0 2.49E-053.53E-03 8.14E-07
+01 03
PERE = Use of renewable primary energy excluding renewable primary energy resources used as raw materials; PERM = Use of renewable primary
energy resources used as raw materials; PERT = Total use of renewable primary energy resources; PENRE = Use of non-renewable primary energy
excluding non-renewable primary energy resources used as raw materials; PENRM = Use of non-renewable primary energy resources used as raw
materials; PENRT = Total use of non-renewable primary energy resources; SM = Use of secondary material; RSF = Use of renewable secondary fuels;
NRSF = Use of non-renewable secondary fuels; FW = Use of net fresh water
RESULTS OF THE LCA – WASTE CATEGORIES AND OUTPUT FLOWS according to EN 15804+A2:
1 piece average overhead shower incl. packaging
Parameter Unit A1-A3 A4 A5 B1 B2 B3 B4 B5 B6/1 B6/2 B7 C1 C2 C3 C4 D
-4.08E-
HWD kg 2.12E-059.52E-11 6.7E-11 0 8.5E-03 0 0 0 3.84E-068.38E-061.21E-07 0 2E-11 2.12E-10 1.2E-11
09
2.25E 9.38E -6.84E-
NHWD kg 4.1E-01 3.63E-04 3.3E-03 0 6.58E-01 0 0 0 2.7E+00 0 5.96E-051.05E-018.38E-02
+01 +01 03
4.72E -5.08E-
RWD kg 2.62E-034.14E-061.52E-05 0 4.13E-03 0 0 0 4.53E-02 4.82E-02 0 6.89E-075.19E-057.73E-07
+00 04
CRU kg 0 0 0 0 0 0 0 0 0 0 0 0 0 0 0 0
MFR kg 0 0 5.73E-01 0 0 0 0 0 0 0 0 0 0 0 0 0
MER kg 0 0 0 0 0 0 0 0 0 0 0 0 0 0 0 0
2.97E
EEE MJ 4.87E-02 0 1.56E-01 0 0 0 0 0 0 0 0 0 0 3.04E-05 0
+00
5.36E
EET MJ 1.01E-01 0 2.81E-01 0 0 0 0 0 0 0 0 0 0 0 0
+00
HWD = Hazardous waste disposed; NHWD = Non-hazardous waste disposed; RWD = Radioactive waste disposed; CRU = Components for re-use;
MFR = Materials for recycling; MER = Materials for energy recovery; EEE = Exported electrical energy; EET = Exported thermal energy
RESULTS OF THE LCA – additional impact categories according to EN 15804+A2-optional:
1 piece average overhead shower incl. packaging
Parameter Unit A1-A3 A4 A5 B1 B2 B3 B4 B5 B6/1 B6/2 B7 C1 C2 C3 C4 D
Disease 3.01E- 5.44E- 3.88E- 3.31E- 5.09E- 3.13E- 1.58E- 2.97E- 3.14E- 1.52E-
PM 0 0 0 0 0 -9.9E-09
incidence 07 08 10 06 06 05 06 10 09 10
kBq U235 7.44E- 6.02E- 1.73E- 2.14E 7.21E 7.74E 7.59E 1.01E- 5.09E- -5.17E-
IR 0 0 0 0 0 1.11E-04
eq 01 04 03 +00 +00 +02 +00 04 03 02
1.68E 1.96E 2.81E 1.33E 8.29E 2.81E- 9.18E- -2.95E
ETP-fw CTUe 1.8E-01 0 2E+02 0 0 0 0 3.9E-02
+02 +00 +02 +04 +03 01 01 +00
3.31E- 5.25E- 2.21E- 3.77E- 2.81E- 5.68E- 2.57E- -1.69E-
HTP-c CTUh 3.85E-11 0 0 0 0 6E-08 0 2.3E-11
07 12 08 07 07 12 12 10
4.05E- 1.96E- 2.44E- 7.49E- 6.34E- 1.42E- 2.89E- 3.02E- 2.08E- 2.38E- -7.56E-
HTP-nc CTUh 0 0 0 0 0
07 09 10 07 06 05 05 10 09 10 09
5.79E 1.29E- 3.18E 2.86E- 4.87E- -8.61E
SQP SQP 5.7E-01 0 0 0 0 1.2E+02 1E+04 2.9E+02 0 1.3E-01
+01 01 +02 01 03 +00
PM = Potential incidence of disease due to PM emissions; IR = Potential Human exposure efficiency relative to U235; ETP-fw = Potential comparative
Toxic Unit for ecosystems; HTP-c = Potential comparative Toxic Unit for humans (cancerogenic); HTP-nc = Potential comparative Toxic Unit for humans
(not cancerogenic); SQP = Potential soil quality index
Disclaimer 1 – for the indicator “Potential Human exposure efficiency relative to U235”. This impact category deals mainly with the
eventual impact of low-dose ionizing radiation on human health of the nuclear fuel cycle. It does not consider effects due to possible
nuclear accidents, occupational exposure or radioactive waste disposal in underground facilities. Potential ionizing radiation from the
soil, radon and from some construction materials is also not measured by this indicator.
Disclaimer 2 – for the indicators “abiotic depletion potential for non-fossil resources”, “abiotic depletion potential for fossil resources”,
“water (user) deprivation potential, deprivation-weighted water consumption”, “potential comparative toxic unit for ecosystems”,
“potential comparative toxic unit for humans – cancerogenic”, “Potential comparative toxic unit for humans - not cancerogenic”,
“potential soil quality index”. The results of this environmental impact indicator shall be used with care as the uncertainties on these
results are high as there is limited experience with the indicator.
6. LCA: Interpretation
8 Environmental Product Declaration - Hansgrohe Group - Overhead Showers
The dominance analysis shows that the results, all products were balanced and compared to the
modules B2, B6 and B7 are the dominant life cycle stages in average product
most of the weighted by production volume.
categories. The contribution of B2 is due to the demand of soap
and water for
cleaning. Module B6 dominates most of the indicators due to
the energy demand The different types of products all
for water heating and module B7 has a high contribution to have the same function and differ mainly in terms of design,
EPfreshwater which has an
due to the wastewater treatment. The module A1-A3 has a very influence on construction and materials used. The basic
low contribution structure of the
to all categories except of ADPE. In this indicator the provision product types is always similar. Material type and quantity
of brass and proportions do not
zinc has the largest contribution. The end of life stage has no differ much, as also shown in the average material composition
significant table.
influence on the environmental indicators.
The deviation of the GWP fossil in
The environmental burdens from the modules A1-C4 has a maximum of 106% and a minimum of -
transports (modules A4 and C2) account for less than 1% of the 59% with scenario B6/1
total burdens of (gas low temperature boiler). The deviation of the GWP fossil in
the respective indicators in all cases. modules A1-C4
has a maximum of 106% and a minimum of -60% with scenario
B6/2 (electric
instantaneous water heater).
The possible potentials of avoided
loads of subsequent systems (module D) lie outside the
considered system
boundaries and relate exclusively to credits from recycling and For an average scenario, where 50%
thermal of water is heated with gas low temperature boiler and 50%
recycling by means of incineration with energy recovery of the with electric
different materials. instantaneous water heater, 52% of the overhead showers
produced are above the
average GWP fossil value. Whereas 48% reflect the average or
are lower than the
374,764 overhead showers of 179 average. However, 75% of the ones which are above the
different product types were produced. For the assessment of average just deviate
the variability of between +10 and +32 %.
9 Environmental Product Declaration - Hansgrohe Group - Overhead Showers
B7. The higher the
deviation from the average GWP, the higher the flow rate. The
Modules flow rate ranges
B6 and B7 account for more than 90% of the GWP fossil between 5.4 and 28.1 l/min. Consequently, the production
indicator. The deviation phase has a minor
from the average is mainly caused by the flow rate in module influence on the LCA results.
7. Requisite evidence
The drinking water regulation determines the quality of drinking • Thermoplastic elastomers: Recommendation for the
water at the point of withdrawal. This result in requirements for hygienic assessment of products made of thermoplastic
used materials in drinking water installations in general and elastomers in contact with drinking water (TPE transition
therefore in sanitary fittings in particular. recommendation)
All materials used by Hansgrohe SE, which are in contact with • Ceramics: draft assessment basis for enamels and
drinking water, fulfill the drinking water regulation. ceramic materials: assessment basis for enamels and
Regulations for metals (Europe-wide): ceramic materials in contact with drinking water
(enamel/ceramic assessment basis)
• Acceptance of metallic materials used for products in
• Lubricants: Guideline for the hygienic assessment of
contact with drinking water: 4MS Common Approach
lubricants in contact with drinking water (sanitary
- Part A – Procedure for the acceptance
lubricants), (Lubricant Guideline)
- Part B – 4MS Common Composition List
Regulation for other materials (France):
• Metal recommendation of the federal environment
• ACS: Attestation de Conformité Sanitaire (plastics,
agency: metal materials suitable for drinking water
elastomers, metals)
hygiene
Regulation for other materials (UK):
Regulations for other materials (Germany):
• BS 69 20: Suitability of non-metallic products for use in
• KTW: Assessment basis for plastics and other organic
contact with water intended for human consumption with
materials in contact with drinking water
regard to their effect on the quality of water (plastics,
• Elastomer guideline: Guideline for the hygienic
elastomers)
assessment of elastomers in contact with drinking water
Products of the Hansgrohe SE are therefore uncritical to use
with any drinking water.
8. References
Standards DIN EN ISO 14025: Environmental labels and declarations -
Type III environmental declarations - Principles and procedures,
2011-10
EN 1112
EN 1112:2008 Sanitary tapware - Shower outlets for sanitary
tapware for water supply systems of type 1 and type 2 - EN 15804
General technical specification DIN EN 15804:2012+A2:2019+AC:2021: Sustainability of
ISO 3822 construction works - Environmental product declarations - Core
ISO 3822: Acoustics – Laboratory tests on noise emission from rules for the product category of construction products
appliances and equipment used in water supply installations
DIN EN ISO 45001
DIN 4102-1 DIN EN ISO 45001:2018: Occupational health and safety
DIN 4102-1: Fire behaviour of building materials and building management systems — Requirements with guidance for use.
components - Part 1: Building materials; concepts, 2018-03
requirements and tests. 1998-05
DIN EN ISO 50001
DIN EN ISO 9001 DIN EN ISO 50001:2018: Energy management systems —
DIN EN ISO 9001:2015: Quality management systems - Requirements with guidance for use. 2018-08
Requirements (ISO 9001:2015)
Further References
DIN EN 13501-1
DIN EN 13501-1:2019-05: Fire classification of construction
products and building elements - Part 1: Classification using AVV
data from reaction to fire tests; German version EN 13501- Draft General administrative provision relating to the Order on
1:2018 the European list of wastes (Waste List Order – German
designation: AVV) of 10 December 2001.
DIN EN ISO 14001
DIN EN ISO 14001:2015, Environmental management systems ECHA
— Requirements with guidance for use, 2015-09 European Chemicals Agency (ECHA) Candidate List of
Substances of Very High Concern (SVHC) for Authorisation
https://echa.europa.eu/de/candidate-listtable
DIN EN ISO 14025
10 Environmental Product Declaration - Hansgrohe Group - Overhead Showers
General
Ecoinvent Instructions for the EPD programme of Institut Bauen und
ecoinvent 3.6 Database on Life Cycle Inventories (Life Cycle Umwelt e.V.
Inventory data), ecoinvent Association, Zürich, 2020 Version 2.0, Berlin: Institut Bauen und Umwelt e.V., 2021,
www.ibu-epd.com
EU Ordinance on biocide Products No. 528/2012
European Parliament, 2012. Regulation (EU) no 528/2012 of PCR Part A
the European parliament and of the council of 22 May 2012 Institut
concerning the making available on the market and use of Bauen und Umwelt e.V. (IBU), Product Category Rules for
biocidal products Building-Related Products and Services. Part A: Calculation
rules for
the life cycle assessment and requirements on the project
report.
Version 2.1, Berlin, 11/2021
Eurostat
PCR Part B
Institut Bauen und Umwelt e.V. (IBU), Requirements on the
EPD for fittings and showers. Version 1.1, Berlin, 03/2022
Eurostat, last update 26/10/2021 on
https://ec.europa.eu/eurostat/databrowser/view/ten00063/default/table?Thünen Institute
ang=en
Diestel, Sylvia / Weimar, Holger: Der Kohlenstoffgehalt in
Holz- und Papierprodukten - Herleitung und
Umrechnungsfaktoren. Thünen
GaBi Working Paper 38. Johann Heinrich von Thünen-Institut.
GaBi Hamburg, 2014
10.6, GaBi Software System and Database for Life Cycle The literature referred to in the Environmental Product
Engineering version 2021.2, Sphera Solutions GmbH, Declaration must be listed in full.Standards already fully quoted
Leinfelden-Echterdingen, 1992-2021 in the EPD do not need to be listed here again.
The current version of PCR Part A and PCR Part B of the PCR
document on which they are based must be referenced.
IBU 2021
11 Environmental Product Declaration - Hansgrohe Group - Overhead Showers
Publisher
Institut Bauen und Umwelt e.V. +49 (0)30 3087748- 0
Hegelplatz 1 info@ibu-epd.com
10117 Berlin www.ibu-epd.com
Germany
Programme holder
Institut Bauen und Umwelt e.V. +49 (0)30 3087748- 0
Hegelplatz 1 info@ibu-epd.com
10117 Berlin www.ibu-epd.com
Germany
Author of the Life Cycle Assessment
brands & values GmbH +49 421 70 90 84 33
Altenwall 14 info@brandsandvalues.com
28195 Bremen www.brandsandvalues.com
Germany
Owner of the Declaration
Hansgrohe Group +49 7836 51-0
Auestr. 5-9 info@hansgrohe-group.com
77761 Schiltach www.hansgrohe-group.com
Germany
12 Environmental Product Declaration - Hansgrohe Group - Overhead Showers
