ENVIRONMENTAL PRODUCT DECLARATION
as per ISO 14025 and EN 15804+A1
Owner of the Declaration Isolparma
Programme holder Institut Bauen und Umwelt e.V. (IBU)
Publisher Institut Bauen und Umwelt e.V. (IBU)
Declaration number EPD-ISL-20200304-CBA2-EN
Issue date 18.12.2020
Valid to 17.12.2025
ISOLPARMA RF2 average thick panel
Isolparma
www.ibu-epd.com | https://epd-online.com
Umwelt Produktdeklaration Name des Herstellers – Name des Produkts
General Information
Isolparma ISOLPARMA RF2 insulation panel
Programme holder Owner of the declaration
IBU – Institut Bauen und Umwelt e.V. Isolparma
Panoramastr. 1 Piazza L. Da Porto, n. 14
10178 Berlin
Germany 35131 | Padova | PD | Italy
Declaration number Declared product / declared unit
EPD-ISL-20200304-CBA2-EN ISOLPARMA RF2 expanded rigid polyurethane foam ,
covered on both sides by bituminous paper facers, and
produced by Isolparma. The EPD applies to 1 m2 of an
average 75 mm thick PIR sandwich board, i.e. 0.075
m3, with an average density between foam and facing
of 31.3 kg/m3.
This declaration is based on the product Scope:
category rules: Isolparma srl produces ISOLPARMA RF2 that is a
Insulating materials made of foam plastics, 06.2017 high performance insulation board manufactured
(PCR checked and approved by the SVR) from closed cell expanded rigid polyurethane
foam, covered on both sides by bituminous paper
facers.The data have been provided by the only
Issue date
Isolparma factory that was located in Padova (Italy)
18.12.2020
for the year 2019.The owner of the declaration shall
be liable for the underlying information and
Valid to evidence; the IBU shall not be liable with respect to
17.12.2025 manufacturer information, life cycle assessment
data and evidences
The owner of the declaration shall be liable for the
underlying information and evidence; the IBU shall not
be liable with respect to manufacturer information, life
cycle assessment data and evidences.
The EPD was created according to the specifications
of EN 15804+A1. In the following, the standard will be
simplified as EN 15804.
Verification
The standard EN 15804 serves as the core PCR
Independent verification of the declaration and data
according to ISO 14025:2010
Dipl. Ing. Hans Peters internally x externally
(chairman of Institut Bauen und Umwelt e.V.)
Dr. Alexander Röder Prof. Dr. Birgit Grahl
(Managing Director Institut Bauen und Umwelt e.V.)) (Independent verifier)
Product
Product description/Product definition 13165:2012+A2:2016 Thermal insulation products for
Isolparma’s thermo insulation panels are mainly used buildings - Factory made rigid polyurethane foam (PU)
in the building/construction sector and that of industrial products - Specification.
insulation. This EPD refers to RF2 Average thick panel, made of
The panels are made of thermo-setting closed cells an insulation component in polyurethane foam using
polyurethane foam (PU) supplied with various types of blowing agent Pentane-based, covered on both sides
flexible facers on both sides of the panel. The by bituminous paper.
nature/type of facercontributes to the performance
characteristics of the product and its application. The panel is produced in standard dimensions of 600 x
Expanded rigid polyurethane foam is distinguished by 1200 mm and straight finish borders. Upon request
its’ excellent thermo insulation performance, and for minimum quantities, the panels may be
mechanical resistance, workability, lightness, and produced in various dimensions. RF2 Average thick
durability. panel is produced by a certified company with
The performance of Isolaprama's panels is determined systems: ISO 9001, ISO 45001, ISO 14001 in its entire
based on the European norm EN line of products.
2 Environmental Product Declaration Isolparma srl – Isolparma RF2
 This product/article/at least one partial article
For the placing on the market of the product in the contains substances listed in the candidate
EuropeanUnion/European Free Trade Association
list (date: 17.11.2020) exceeding 0.1
(EU/EFTA) (with the exception of Switzerland) the
percentage by mass: no
Regulation (EU) No. 305/2011 (CPR) applies. The
product needs a Declaration of Performance taking  This product/article/at least one partial article
into consideration EN 13165:2012+A2:2016 Thermal doesn’t contain other CMR substances in
insulation products for building- factory made rigid categories 1A or 1B which are not on the
polyurethane foam (PU) products - Specification and candidate list, exceeding 0.1 percentage by
the CE-marking. For the application and use the
mass: no
respective national provisions apply.
 Biocide products were added to this
Application
construction product or it has been treated
The ISOLPARMA RF2 panel is suited for walk-on
roofs, paved roofs and foor insulation. with biocide products (this then concerns a
treated product as defined by the (EU)
Technical Data Ordinance on Biocide Products No.
The data provided by the Declaration of Performance 528/2012): no
apply. In this Life Cycle Assessment, a PU insulation
board with the following properties has been regarded:
Additional declaration according to quoted law: The
Constructional data product is compliant with all requirements indicated at
Name Value Unit chapter 2.4.2.9 of the PANGPP 2017:
Gross density 31.3 kg/m3  Any blowing agent with Ozone depletion
Declared average Thermal potential >0 is not used in production
0.027 W/mK
conductivity λD acc. to /EN 13165/  Catalysts lead-based are not used in
Compressive strength at 10% > 150 kPa production
deformation acc. to /EN 826/
 Flame retardants used in production
Tensile strength perpendicular to the
> 40 kPa (belonging to the Organophosphorus class)
face acc. to /EN 1607/
are not banned by any national or European
Water absorption by total immersion
< 5 Vol.-%
acc. to /EN 12087/ regulation
Water absorption by partial immersion  According to the raw materials declarations of
< 0.3 kg/m²
acc. to /EN 1609/ suppliers the minimum amount of recycled
Water vapour diffusion resistance 87 raw materials based on the insulation board
factor μ acc. to /EN 12086/
(PU foam and facers) weight is 3 %w and the
Euroclass reaction to fire acc. to /EN
F minimum amount of recycled raw materials
11925/
based on the PU insulation foam weight is 4
This provides a thermal resistance R = 2.73 m² k/W. %w (note: this information is not explicitly
considered in the LCA and not included in the
EPD tables that only refer to recycling content
in the foreground system).
Base materials/Ancillary materials
Core material (about 78.8 % of the weight of the
declared unit):
Reference service life
Closed-cell Polyiso (PIR) rigid foam made from MDI
The durability of insulation panels is normally at least
(50-65 %), polyols (20-30 %), pentane (4-5 %) and
as long as the lifetime of the building in which it is
additives (4-7 %).
used. The experimental data show that the reference
Facing (about 26,1 % of the weight of the declared
life is longer than 50 years, Clima 2019.
unit): bituminous paper consisting of kraft paper (60-
70%) and bitumen (40-30%).
The PU board for insulation:
LCA: Calculation rules
Declared Unit conductivity λD
The declared unit is 1 m² with an average thickness of Layer thickness 0.075 m
75 mm, e. g. 0.075 m³. Corresponding conversion Conversion factor to 1 kg 2.35 kg/m²
factors are listed in the table below. Weight of declared unit 2.35 kg/m²
This provides a thermal resistance R = 2.73 m2K/W.
Declared unit
Name Value Unit The LCI data used in this report refer to an average
Declared unit 1 m2 product having an average thickness (material in the
Gross density 31.3 kg/m3 repipes of different thicknesses are weighted according
Volume 0.075 m³ to the relative production in square meters). The type
Grammage 2.35 kg/m2 of declaration is 1 c - declaration of an average product
Declared average thermal 0.027 W/mK
3 Environmental Product Declaration Isolparma srl – Isolparma RF2
from a manufacturer's plant. recovery, landfill)
D - Benefits and loads beyond system boundary
Comparability
Basically, a comparison or an evaluation of EPD data
System boundary is only possible if all the data sets to be compared
This life cycle assessment for the production of the were created according to EN 15804 and the building
polyurethane insulation board considers the life cycle context, respectively the product-specific
from the supply of raw materials to the manufacturer´s characteristics of performance, are taken into account.
gate (cradle-to-gate with options). It also includes the
transport to the construction site, the installation and For life cycle modelling of the considered products,
the end-of-life stage of the used PU thermal insulation the /GaBi 9 2020 has been used.
board. The life cycle is split into the following individual
phases:
A1 - Raw material formulation
A2 - Raw material transport
A3 - Production of the insulation board and packaging
material
A4 - Transport to the construction site
A5 - Emissions and cutting losses during installation
and packaging disposal
C2 - Transport to end of life
C3/C4 - End-of-Life: waste management (thermal
LCA: Scenarios and additional technical information
Water consumption - m3
Auxiliary - kg
Transport to the building site (A4) Other resources - kg
The distances calculated are weighted average Electricity consumption - kWh
distances according to the overall sales distribution; Other energy carriers - MJ
such distribution is considered similar for all Isolparma Material loss - kg
products.
Name Value Unit
Replacement (B4) / Refurbishment (B5)
Truck with a capacity of 17.3 tons 270 km
Name Value Unit
F dwer tr y p aw yi lt oh a a d c ca ap pa ac ci it ty y of 1200-10000 124 km Replacement cycle - Nu Rm Sb Ler/
Ship with a capacity of 27500 dwt
11000 km Electricity consumption - kWh
payload capacity tons
Litres of fuel - l/100km
Plane with a capacity of 22 ton 0 km
Replacement of worn parts - kg
Installation into the building (A5)
Name Value Unit
Reference service life
Material loss 0.0469 kg
Name Value Unit
VOC in the air Pentane 1.27E-06 kg Reference service life - a
Life Span (according to BBSR) - a
Life Span according to the
Use or application of the installed product (B1) see - a
manufacturer
section 2.12 "Use"
Declared product properties (at the
Name Value Unit - -
gate) and finishes
Design application parameters (if
Maintenance (B2)
instructed by the manufacturer),
Name Value Unit
including the references to the - -
Information on maintenance - -
appropriate practices and application
Number/
Maintenance cycle - codes
RSL
An assumed quality of work, when
Water consumption - m3
installed in accordance with the - -
Auxiliary - kg
manufacturer’s instructions
Other resources - kg
Outdoor environment, (for outdoor
Electricity consumption - kWh
applications), e.g. weathering,
Other energy carriers - MJ
pollutants, UV and wind exposure, - -
Material loss - kg building orientation, shading,
temperature
Repair (B3) Indoor environment (for indoor
Name Value Unit applications), e.g. temperature, - -
Information on the repair process - - moisture, chemical exposure
Information on the inspection process - - Usage conditions, e.g. frequency of
Repair cycle - Number/ use, mechanical exposure - -
RSL Maintenance e.g. required frequency, - -
4 Environmental Product Declaration Isolparma srl – Isolparma RF2
type and quality and replacement of
components
Operational energy use (B6) and Operational water
use (B7)
Name Value Unit
Water consumption - m3
Electricity consumption - kWh
Other energy carriers - MJ
Equipment output - kW
End of life (C1-C4)
The results for the end-of-life are declared for the 2
different scenarios:
Name Value Unit
Scenario No 1: Material Incineration 100 %
Scenario No 2: Landfill 100 %
C4: Disposal scenarios used is divided into the 2
sub-scenarios:
1) Incineration 100% (C4/1)
2) Landfilling 100% (C4/2)
D: Benefits and loads beyond system boundary is
divided into the 2 sub-scenarios:
1) Incineration 100% (D1)
2) Landfilling 100% (D2)
Reuse, recovery and/or recycling potentials (D),
relevant scenario information
Name Value Unit
Module D includes credits from recycling materials of
insulation panels and packaging, energy credits from
thermal recovery of the packaging. The results are
declared for the same 3 different scenarios described
above.
5 Environmental Product Declaration Isolparma srl – Isolparma RF2
LCA: Results
The tables below show the results of the LCA. Basic information on all declared modules provides chapter 4.
There are two scenarios for the end-of-life (C3, C4 and D) analyzed: Scenario 1 considers 100% incineration,
Scenario 2 considers 100% landfill disposal.
For SM, RSF, NRSF,CRU indicators only the foreground system is considered.
DESCRIPTION OF THE SYSTEM BOUNDARY (X = INCLUDED IN LCA; MND = MODULE NOT DECLARED;
MNR = MODULE NOT RELEVANT)
BENEFITS AND
CONSTRUCTI LOADS
PRODUCT STAGE ON PROCESS USE STAGE END OF LIFE STAGE BEYOND THE
STAGE SYSTEM
BOUNDARIES
6 Environmental Product Declaration Isolparma srl – Isolparma RF2
lairetam
waR
ylppus tropsnarT
gnirutcafunaM
eht
morf
tropsnarT
etis
eht
ot
etag
ylbmessA esU
ecnanetniaM
riapeR
tnemecalpeR tnemhsibrufeR
ygrene
lanoitarepO esu
retaw
lanoitarepO esu
noitcurtsnoc-eD
noitilomed tropsnarT
gnissecorp
etsaW
lasopsiD -esueR -yrevoceR -gnilcyceR laitnetop
A1 A2 A3 A4 A5 B1 B2 B3 B4 B5 B6 B7 C1 C2 C3 C4 D
X X X X X MND MND MNR MNR MNR MND MND MND X X X X
RESULTS OF THE LCA - ENVIRONMENTAL IMPACT according to EN 15804+A1: 1 m² RF2 insulation panel
Parameter Unit A1-A3 A4 A5 C2 C3/1 C3/2 C4/1 C4/2 D/1 D/2
GWP [kg CO2-Eq.] 5.37E+0 4.44E-2 8.71E-1 1.10E-2 0.00E+0 0.00E+0 4.47E+0 3.58E+1 -2.01E+0 -1.46E+0
ODP [kg CFC11-Eq.] 8.34E-6 9.77E-18 1.67E-7 2.74E-18 0.00E+0 0.00E+0 2.63E-15 1.32E-14 -4.25E-14 -4.28E-14
AP [kg SO2-Eq.] 1.21E-2 4.04E-4 5.27E-4 2.42E-5 0.00E+0 0.00E+0 1.88E-3 1.29E-2 -3.32E-3 -3.02E-3
EP [kg (PO4)3--Eq.] 2.38E-3 5.41E-5 1.34E-3 5.87E-6 0.00E+0 0.00E+0 4.53E-4 6.43E-2 -3.89E-4 -3.35E-4
POCP [kg ethene-Eq.] 1.03E-2 -7.64E-6 3.85E-4 -7.79E-6 0.00E+0 0.00E+0 1.20E-4 8.86E-3 -2.66E-4 -2.17E-4
ADPE [kg Sb-Eq.] 1.12E-5 3.40E-9 2.44E-7 1.01E-9 0.00E+0 0.00E+0 1.13E-7 7.48E-7 -5.05E-7 -4.82E-7
ADPF [MJ] 1.30E+2 5.89E-1 3.78E+0 1.49E-1 0.00E+0 0.00E+0 2.04E+0 5.27E+1 -2.63E+1 -1.67E+1
GWP = Global warming potential; ODP = Depletion potential of the stratospheric ozone layer; AP = Acidification potential of land and water; EP =
Caption Eutrophication potential; POCP = Formation potential of tropospheric ozone photochemical oxidants; ADPE = Abiotic depletion potential for non-
fossil resources; ADPF = Abiotic depletion potential for fossil resources
RESULTS OF THE LCA - INDICATORS TO DESCRIBE RESOURCE USE according to EN 15804+A1: 1 m²
RF2 insulation panel
Parameter Unit A1-A3 A4 A5 C2 C3/1 C3/2 C4/1 C4/2 D/1 D/2
PERE [MJ] 2.34E+1 IND 6.11E-1 IND IND IND 6.48E-1 IND IND IND
PERM [MJ] 2.21E+0 IND 0.00E+0 IND IND IND 0.00E+0 IND IND IND
PERT [MJ] 2.56E+1 2.69E-2 6.11E-1 8.63E-3 0.00E+0 0.00E+0 6.48E-1 4.25E+0 -1.13E+1 -1.14E+1
PENRE [MJ] 6.18E+1 IND 2.95E+0 IND IND IND 7.68E+1 IND IND IND
PENRM [MJ] 7.60E+1 IND -1.72E+0 IND IND IND -7.43E+1 IND IND IND
PENRT [MJ] 1.38E+2 5.92E-1 1.22E+0 1.50E-1 0.00E+0 0.00E+0 2.54E+0 5.47E+1 -3.60E+1 -2.65E+1
SM [kg] 0.00E+0 0.00E+0 0.00E+0 0.00E+0 0.00E+0 0.00E+0 0.00E+0 0.00E+0 0.00E+0 0.00E+0
RSF [MJ] 0.00E+0 0.00E+0 0.00E+0 0.00E+0 0.00E+0 0.00E+0 0.00E+0 0.00E+0 0.00E+0 0.00E+0
NRSF [MJ] 0.00E+0 0.00E+0 0.00E+0 0.00E+0 0.00E+0 0.00E+0 0.00E+0 0.00E+0 0.00E+0 0.00E+0
FW [m³] 6.01E-2 3.16E-5 1.43E-3 1.01E-5 0.00E+0 0.00E+0 1.07E-2 5.49E-3 -1.31E-2 -1.32E-2
PERE = Use of renewable primary energy excluding renewable primary energy resources used as raw materials; PERM = Use of
renewable primary energy resources used as raw materials; PERT = Total use of renewable primary energy resources; PENRE = Use of
non-renewable primary energy excluding non-renewable primary energy resources used as raw materials; PENRM = Use of non-
Caption
renewable primary energy resources used as raw materials; PENRT = Total use of non-renewable primary energy resources; SM = Use
of secondary material; RSF = Use of renewable secondary fuels; NRSF = Use of non-renewable secondary fuels; FW = Use of net fresh
water
RESULTS OF THE LCA – WASTE CATEGORIES AND OUTPUT FLOWS according to EN 15804+A1:
1 m² RF2 insulation panel
Parameter Unit A1-A3 A4 A5 C2 C3/1 C3/2 C4/1 C4/2 D/1 D/2
HWD [kg] 1.08E-5 2.13E-8 2.20E-7 6.93E-9 0.00E+0 0.00E+0 2.79E-9 2.01E-7 -1.42E-8 -1.09E-8
NHWD [kg] 1.23E-1 8.64E-5 9.13E-1 2.37E-5 0.00E+0 0.00E+0 2.25E-1 4.47E+1 -1.96E-2 -1.83E-2
RWD [kg] 2.93E-3 9.94E-7 8.09E-5 2.76E-7 0.00E+0 0.00E+0 1.98E-4 7.93E-4 -3.85E-3 -3.88E-3
CRU [kg] 0.00E+0 0.00E+0 0.00E+0 0.00E+0 0.00E+0 0.00E+0 0.00E+0 0.00E+0 0.00E+0 0.00E+0
MFR [kg] 0.00E+0 0.00E+0 1.37E-2 0.00E+0 0.00E+0 0.00E+0 0.00E+0 0.00E+0 0.00E+0 0.00E+0
MER [kg] 0.00E+0 0.00E+0 1.56E-2 0.00E+0 0.00E+0 0.00E+0 2.35E+0 0.00E+0 0.00E+0 0.00E+0
EEE [MJ] 0.00E+0 0.00E+0 3.39E-1 0.00E+0 0.00E+0 0.00E+0 1.25E+1 1.26E+1 0.00E+0 0.00E+0
EET [MJ] 0.00E+0 0.00E+0 1.56E-1 0.00E+0 0.00E+0 0.00E+0 7.85E+0 0.00E+0 0.00E+0 0.00E+0
HWD = Hazardous waste disposed; NHWD = Non-hazardous waste disposed; RWD = Radioactive waste disposed; CRU = Components
Caption for re-use; MFR = Materials for recycling; MER = Materials for energy recovery; EEE = Exported electrical energy; EET = Exported
thermal energy
References
Standards ISO 9001:2015 Quality management
EN 15804 ISO 14001
EN 15804:2012-04+A1 2013, Sustainability of ISO 14001: 2015 Environmental management
construction works — Environmental Product systems
Declarations — Core rules for the product category of
construction products. ISO 45001
ISO 45001: 2018 Occupational health and safety
ISO 14025 management systems
EN ISO 14025:2011-10, Environmental labels and
declarations — Type III environmental declarations —
Principles and procedures. BNB
Bewertungssystem Nachhaltiges Bauen (en:
IBU 2016 assessment system sustainable building)
Institut Bauen und Umwelt e.V.: General Programme https://www.bbsr.bund.de/BBSR/EN/RP/FutureBuilding
Instructions for the Preparation of EPDs at the Institut /2SustainableBuildingQuality/2009/ServiceLife/01_Star
Bauen und Umwelt e.V. Version 1., Berlin: Institut t_dossier.html?nn=391866&notFirst=true&docId=3909
Bauen und Umwelt e.V., 2016. 00
www.ibu-epd.com
Candidate List
EN 13165 https://echa.europa.eu/it/candidate-list-table (date
EN 13165:2012+A2:2016 Thermal insulation products 17.11.2020)
for buildings -
Factory made rigid polyurethane foam (PU) products - Clima 2019
Specification Clima 2019 PaperPolyurethane
“Environmental Impacts for a Polyurethane Panel”
EN 826 E. Guolo, F. Cappelletti, P. Romagnoni, F. Raggiotto
EN 826:2013 Determination of Compression Behavior
of Thermal Insulation Products GaBi 9 2020
GaBi 9: Documentation of GaBi 9: Software-System
EN 1607 and Database for Life Cycle Engineering. Copyright,
EN 1607: 2013 Thermal insulating products for TM. Stuttgart, Leinfelden-Echterdingen, 1992-2020
building applications. Determination of tensile strength http://www.gabi-software.com
perpendicular to faces
PANGPP 2017
EN 12087 Piano d’ Azione Nazionale sul Green Public
EN 12087:2013 Procurement (PANGPP) – Gazzetta Ufficiale della
Thermal insulating products for building applications. Repubblica Italiana, Serie Generale n.17, 11-10-2017,
Determination of long term water absorption by http://www.minambiente.it/sites/default/files/archivio/all
immersion. egati/GPP/GPP_CAM_Edilizia.pdf
EN 1609 PCR Part A
EN 1609: for Building-Related Products and Services.
Thermal insulating products for building applications. Part A: Calculation Rules for the Life Cycle
Determination of short term water absorption by partial Assessment and Requirements on the Background
immersion. Report. Version 06.2017
EN 12086 PCR Part B
EN 12086: 2013 PCR Guidance-Texts for Building-Related Products
Thermal insulating products for building applications. and Services; Part B: Requirements on the EPD for
Determination of water vapour transmission properties. Insulating materials made of foam plastics; Institute
Construction and Environment e.V. (IBU). Version
EN 11925 06.2017
EN 11925:2010 https://epd-online.com
Reaction to fire tests. Ignitability of products subjected
to direct impingement of flame. Single-flame source REACH
test. REACH Registration, Evaluation, Authorization and
Restriction of Chemical, 2007
ISO 9001
7 Environmental Product Declaration Isolparma srl – Isolparma RF2
Publisher
Institut Bauen und Umwelt e.V. Tel +49 (0)30 3087748- 0
Panoramastr. 1 Fax +49 (0)30 3087748- 29
10178 Berlin Mail info@ibu-epd.com
Germany Web www.ibu-epd.com
Programme holder
Institut Bauen und Umwelt e.V. Tel +49 (0)30 - 3087748- 0
Panoramastr 1 Fax +49 (0)30 – 3087748 - 29
10178 Berlin Mail info@ibu-epd.com
Germany Web www.ibu-epd.com
Author of the Life Cycle
Assessment Tel +39 0544 467132
thinkstep Italy Fax +39 0544 501464
Via Bovini 43 Mail info@thinkstep.com
48123 Ravenna Web www.thinkstep.com
Italy
Owner of the Declaration
Isolparma srl Tel 049 9126213
Piazza Luigi da Porto 14 Fax 049 9129616
35131 Padova Mail info@isolparma.it
Italy Web www.isolparma.it
