ENVIRONMENTAL PRODUCT DECLARATION
as per ISO 14025 and EN 15804+A2
Owner of the Declaration VELUX Group
Publisher Institut Bauen und Umwelt e.V. (IBU)
Programme holder Institut Bauen und Umwelt e.V. (IBU)
Declaration number EPD-VEL-20240208-IBA1-EN
Issue date 23.07.2024
Valid to 22.07.2029
VELUX Commercial continuous rooflights (PC-lysband)
VELUX Group
www.ibu-epd.com | https://epd-online.com
1. General Information
VELUX Group VELUX Commercial continuous rooflights (PC-
lysband)
Programme holder Owner of the declaration
IBU – Institut Bauen und Umwelt e.V. VELUX Group
Hegelplatz 1 Ådalsvej 99
10117 Berlin 2970 Hørsholm
Germany Denmark
Declaration number Declared product / declared unit
EPD­VEL­20240208­IBA1­EN 1 m2 of VELUX Commercial continuous rooflights (PC­lysband)
This declaration is based on the product category rules: Scope:
Windows and doors , 01.08.2021 The LCA represents 100 % of the production volume of VELUX
(PCR checked and approved by the SVR) Commercial continuous rooflights produced by VELUX Commerical in
Kongerslev (DK).
The owner of the declaration shall be liable for the underlying information
Issue date and evidence; the IBU shall not be liable with respect to manufacturer
information, life cycle assessment data and evidences.
23.07.2024
The EPD was created according to the specifications of EN 15804+A2. In
the following, the standard will be simplified as EN 15804.
Valid to
22.07.2029 Verification
The standard EN 15804 serves as the core PCR
Independent verification of the declaration and data according to ISO
14025:2011
internally X externally
Dipl.­Ing. Hans Peters
(Chairman of Institut Bauen und Umwelt e.V.)
Florian Pronold Dr.­Ing. Nikolay Minkov,
(Managing Director Institut Bauen und Umwelt e.V.) (Independent verifier)
1 Environmental Product Declaration ­ VELUX Group ­ VELUX Commercial continuous rooflights (PC­lysband)
2. Product
NPD: no performance declared
2.1 Product description/Product definition
VELUX Commercial continuous rooflights, longlight, are 10 mm, Performance data of the product in accordance with the
20 mm or 30 mm vaulted polycarbonate multiwall rooflights. declaration of performance with respect to its essential
They consist of polycarbonate sheets in multiwall polycarbonate characteristics according to:
material, in combination with aluminium profiles. The are
• EN 14963:2006, Roof coverings - Continuous rooflights
installed on an insulated wooden upstand with plywood on both
of plastics with or without upstands - Classification,
side (sandwich construction).
requirements and test methods
VELUX Commercial continuous rooflights, ridgelight, are 10
mm, 20 mm or 30mm polcarbonate multiwall rooflights in ridge 2.4 Delivery status
shape. They consist of polycarbonate sheets in multiwall
VELUX Commercial continuous rooflights are avilable in widths
polycarbonate material, in combination with aluminium profiles.
ranging from 1600 mm to 2400 mm with a standard with of
The are installed on an insulated wooden upstand with plywood
2000 mm, in lenghts ranging from 1080 mmm do indefininte
on both side (sandwich construction).
with a standard length of 28'800 mm and with upstand heights
For the placing on the market of the product in the European
ranging from 400 mm to 1000 mm with a standard height of 700
Union/European Free Trade Association (EU/EFTA) (with the
mm.
exception of Switzerland) Regulation (EU) No. 305/2011 (CPR)
applies. The product needs a declaration of performance taking 2.5 Base materials/Ancillary materials
into consideration: The delcared product is composed of:
• EN 14963:2006, Roof coverings - Continuous rooflights Name Value Unit
of plastics with or without upstands - Classification, Plywood 43 % ­
requirements and test methods
Aluminium 23 % ­
and the CE­marking.
Polycarbonate (PC) 20 % ­
2.2 Application Sawn timber 13 % ­
VELUX Commercial continuous rooflights are intended for Others 2 % ­
lighting by means of daylight and of ventilating interior spaces
by means of opening devices.
1. This product/article/at least one partial article contains
Areas of application for the VELUX Commercial continuous
substances listed in the ECHA candidate list (date: 15.08.2023)
rooflights are:
exceeding 0.1 percentage by mass: no.
• unheated industrial buildings
• heated industrial buildings 2. This product/article/at least one partial article contains other
• warehouses carcinogenic, mutagenic or reprotoxic (CMR) substances in
• logistics centres categories 1A or 1B which are not on the ECHA candidate list,
• railway stations exceeding 0.1 percentage by mass: not investigated with
• production facilities suppliers.
• sports halls
• shopping centres 3. Biocide products were added to this construction product or it
has been treated with biocide products (this then concerns a
2.3 Technical Data
treated product as defined by the (EU) Ordinance on Biocide
Technical characteristics Products No. 528/2012): no.
Technical characteristics according to DoP No. 457502-11 for
2.6 Manufacture
Polycarbonate Continuous Roof Light, Type HV/RY
All the raw materials including wood, plywood, polycarbonate,
Name Value Unit
acrylic, aluminium, actuators and all ancillary materials (fittings,
Resistance to upward load NPD
screws, glue, plastic parts, gasket, etc.) are bought from
Resistance to downward load NPD external suppliers. First the wood and plywood are cross­cut for
Durability NPD the production of the upstands; in addition, all aluminium parts
Air permeability NPD are cross­cut, drilled and welded; in a last preparatory step, the
polycarbonate and the acrylic are crosscut and shaped. All the
Direct airborne sound insulation acc. EN
22 ­ 23 dB components are then assembled to the final product, which
14963
undergoes a final inspection.
Luminous transmittance (clear) acc. EN 25 % ­ 46
Only a few items are bought manufactured from a sub supplier.
14963 %
That is the aluminium sheets for windscreens and standard
Luminous transmittance (opal) acc. EN 29 % ­ 42 sizes frames for insulated upstands. Also the wood for solid
14963 % frames (Kehlet) is bought from external.
Reaction to fire, wooden frame acc. EN Normally aluminium is not surface treated; sometimes the
D­s2, d0
13501 aluminium parts are painted (wet paint) from a local dealer, but
Reaction to fire, top plate acc. EN 13501 B­s1, d0 not very often.
The insulated upstand made from wood/plywood come usually
Resistance to fire NPD
as laminated material; only in a few cases, the interior side of
External fire performance NPD
the upstands are painted.
Water tighness NPD In order to guarantee the quality assurance of the product,
Small, hard body NPD VELUX operates a quality management system according to
Large, soft body NPD ISO 9001.
Thermal transmittance NPD
2 Environmental Product Declaration ­ VELUX Group ­ VELUX Commercial continuous rooflights (PC­lysband)
utilization scenario is declared in chapter 4.
2.7 Environment and health during manufacturing
The health of employees is protected by suitable measures 2.13 Extraordinary effects
specified by the authorities. These include safety goggles, Fire
hearing protection, helmets, gloves, safety shoes, etc. See table 2.3 for the reaction to fire of the different
Waste generated during every process in the company is components.
collected, sorted and disposed of in a professional and
resource­conserving manner. Water
In the event of unforeseen exposure to water (flood), no
2.8 Product processing/Installation adverse effects on human health or the environment are to be
Continuous rooflight segments consist of an insulated kerb with expected.
pre­assembled top of aluminium profiles and polycarbonate
glazing. The segments are installed on the roof and connected Mechanical destruction
with cover profiles. Fastening of the kerb depends on the sub­ In the event of unforeseen mechanical destruction, VELUX
construction. Watertightening to the roof is done by metal Commercial continous rooflights must be replaced; no adverse
covers or roof membrane with materials brought by the installer. effects on human health or the environment are to be expected.
2.9 Packaging 2.14 Re-use phase
For the transport to the construction site, the VELUX VELUX Commercial continous rooflights can be dismantled
Commercial continuous rooflights are loaded onto a lorry and manually without any problems. The metal parts are usually
fixed with multi­use fastening belts. Usually, no additional recycled, and the wooden and plastic parts are sent for thermal
packaging is used. recycling for energy recovery.
2.10 Condition of use 2.15 Disposal
The material composition of VELUX Commercial continuous VELUX Commercial continous rooflights can be disposed of in
rooflights does not change over their service life. an appropriate landfill. However, due to the value of the
materials or the carbon content of the wooden and plastic parts,
2.11 Environment and health during use
recycling or energy recovery is preferable and common.
VELUX Commercial continuous rooflights do not contain any
pollutants that could be released during use. Waste code according to the European Waste List (Regulation
on the European Waste List):
Environmental protection: According to current knowledge, 17 02 01 wood
hazards to water, air and soil cannot arise when the products 17 02 03 plastics
are used as intended. 17 04 02 aluminium
17 04 05 iron and steel
Health protection: According to current knowledge, no health
hazards or impairments are to be expected. 2.16 Further information
Further documentation on the products, technical data sheets,
2.12 Reference service life
BIM files, etc. can be found at:
It is not possible to calculate the reference service life
according to ISO 15686. The service life based on a www.commercial.velux.com
manufacturer's declaration is 30 years. The corresponding
3. LCA: Calculation rules
For production wastes that are incinerated, it is as­sumed that
3.1 Declared Unit they are incinerated in a municipal waste incineration plant with
1 m2 of VELUX Commercial continuous rooflight is declared. an R­value < 0.6. This means that the incineration process is
considered a waste treatment process and included in the cal
Declared unit and mass reference
culations. The generated 'exported energy' is assumed to have
Name Value Unit
reached the end­of­waste status and is considered in module
Declared unit 1 m2 D.
Grammage 27.7 kg/m2
Module A4 is not declared for being optional. In building
A representative continuous rooflight as longlith of 2000 mm
assessments, the specific transport distance from
widths and 28'800 mm lenghts and a wooden upstand height of
Kongerslev/Denmark to the construction site can be
700 mm is declared. It consists of 3 sheets of polycarbonate (1
considered.
opal, 2 clear) and includes a upstand of insulated wood (64
mm) and 2 flaps and a wind detector.
The products are delivered to the construction site ready to be
installed. Minor impacts from installation, e.g. using cranes, etc.
3.2 System boundary
can be considered insignificant in the light of the total
Type of the EPD: "cradle to gate with modules C1–C4, and
environmental impacts across the life cycle.
module D".
No packaging is used for the transport to the construction site
that would need to be disposed of in module A5. Module A5 is
The production of VELUX Commercial continuous rooflights
not declared for being optional.
(modules A1-A3) includes raw material extraction, energy
generation, waste treatment and all transports up to the factory
Minor impacts from de­installation, e.g. using cranes, etc. can
gate. In accordance with COUNCIL REGULATION (EU) No
be considered insignificant in the light of the total environmental
333/2011, secondary metals are modelled as part of the
impacts across the life cycle. The values of module C1 are
product system from the moment they are available as unmixed
hence 'zero'.
scrap.
3 Environmental Product Declaration ­ VELUX Group ­ VELUX Commercial continuous rooflights (PC­lysband)
Ecoinvent v3.9.1 (2022) with the system model 'allocation – cut­
In the end­of­life, it is assumed that the disassembled products off by classification – unit processes' is used as the background
are brought to a sorting plant for construction materials, where database.
metals and burnable wastes are separeted.
3.6 Data quality
Metals a are recycled; it is assumed that these fractions reach The foreground data are based on extensive and detailed data
end­of­waste state after having been sorted and transported to collection at the production site. The foreground data could be
a recycler. Wooden parts and plastics are incinerated (also due fully linked with corresponding data records from the
to the very limited data availability on plastics recycling and its background database ecoinvent v3.9.1 with the system model
benefits). On average, an average transport distance of 50 km "allocation – cut­off by classification – unit processes".
has been assumed in module C2 with an average lorry for the
transport of the wastes to an incineration plant or to a recycling The background data was updated in 2022. Thus, the quality of
facility. the foreground and background data can be rated as very
good.
The disassembled product is shredded and the materials are
sorted in module C3. The recovered material leaves the The variability of the products consists only in its configuration
product system as 'materials for recycling'. The net amounts of (size). An estimate of the variance of results depending on the
the metals leaving the product system are considered as 'use of size of the products can be found in chapter 7.
secondary material' in Module D.
3.7 Period under review
The wooden parts and the plastics are treated in a waste
incineration plant with an efficiency R1 < 0.6 (according to The LCA data represents the production conditions for the year
CEWEP Energy Report III); the recovered energy is reported as 2022.
'exported energy' and considered in Module D.
3.8 Geographic Representativeness
Land or region, in which the declared product system is
Module C4 is not declared as a "recovery scenario" is assumed
manufactured, used or handled at the end of the product´s
on product level, including waste treatment from
lifespan: Europe
sorting/recycling in module C3.
Module D contains the benefits and loads beyond the system 3.9 Allocation
boundary related to the recycling of metals, which result from
No co­products are generated during the production of the
the treatment of recycled materials from the point of end­of­
VELUX Commercial products. Sorted production scrap of the
waste status to the point of substitution (as loads) and the
different metals, notably aluminium, is considered a secondary
substitution of primary resources (as benefits).
material with no economic value (so no burdens allocated) and
It also includes the benefits and loads related to the energy
considered in the quantification of net flows leaving the product
recovery from plastic and wooden wastes in a municipal waste
system. This approach is chosen to ensure a coherent
incineration plant as modelled in Module C3. Only net flows
quantification of net flows entering module D.
leaving the product system are considered in module D. The
recycled content and the assumed processing losses (e.g.,
Biogenic carbon is allocated based on physical flows
during remelting) are taken from ecoinvent v.3.9.1 datasets.
regardless of the allocation procedure chosen for the process.
The biogenic carbon content of wood products entering or
3.3 Estimates and assumptions
leaving the product system is quantified (manually) as part of
No further assumptions and estimates relevant to the result had
the GWP in conformity with EN 16485.
to be made beyond the points made in chapter 3 and chapter 4.
3.4 Cut-off criteria No processes were modelled as part of the foreground model
that would have required an allocation of multi­input processes.
No data available from the company survey was neglected.
Background datasets on municipal waste incineration plants
These include, among other things, material use, energy
were taken from ecoinvent without any modification.
demand (heat, electricity), packaging materials of raw materials
(insofar as they are generated as waste) and product
Allocation of reuse, recycling and recovery was avoided by the
packaging, consumables in production, waste treatment and
cut­off approach in the foreground model in line with EN 15804.
the transport of all inputs and outputs.
With this approach, mass and energy flows below 1 % were
3.10 Comparability
also accounted for. No processes were neglected that would
Basically, a comparison or an evaluation of EPD data is only
have been known to the project managers and would have
possible if all the data sets to be compared were created
contributed significantly to the indicators of the impact
according to EN 15804 and the building context, respectively
assessment.
the product­specific characteristics of performance, are taken
into account.
3.5 Background data Ecoinvent v3.9.1 (2022) with the system model 'allocation – cut­
off by classification – unit processes' is used as the background
database.
4. LCA: Scenarios and additional technical information
Name ValueUnit
Characteristic product properties of biogenic carbon
kg
Biogenic carbon content in product ­
Information on describing the biogenic carbon content at C
factory gate Biogenic carbon content in accompanying kg
6.41
Note: 1 kg of biogenic carbon is equivalent to 44/12 kg of CO 2. packaging C
4 Environmental Product Declaration ­ VELUX Group ­ VELUX Commercial continuous rooflights (PC­lysband)
Module C1
Inputs and outputs from de­installation are disregared.
Reference service life
Module C2
Name Value Unit
On average, an transport distance of 50 km to a
Life Span according to the sorting/recycling facility and an additional 50 km for sorted
30 a
manufacturer wooden and plastic parts to a municipal waste incineration
The product has passed plant.
Declared product
internal quality controls and
properties (at the gate) and ­
complies with product Module C3
finishes
standard for CE marking A consumption of 0.03 kWh/kg of electricity for shredding and
Design application sorting and 0.437 MJ/kg of diesel fuel for internal logistics are
parameters (if instructed by taken into account to disassemble the product. The recovered
Installation according to
the manufacturer), material leaves the product system as 'materials for recycling'.
assembly instructions and ­
including the references to The net amounts of the metals leaving the product system are
state of the art.
the appropriate practices considered as 'use of secondary material' in Module D.
and application codes
As stated above, it is assumed that 100 % of the wooden and
An assumed quality of
Carried out in accordance plastic parts are treated in a waste incineration plant with an
work, when installed in
with the manufacturer's ­ efficiency R1 < 0.6 (according to CEWEP Energy Report III);
accordance with the
instructions. according to the same source, an efficiency of 31.0 % is
manufacturer’s instructions
assumed for the production of heat and 18.0 % for the
Outdoor environment, (for The declared products are
production of electricity (always referring to the lower heating
outdoor applications), e.g. intended for installation
value of the waste). The recovered energy is reported as
weathering, pollutants, UV outside the building: They are
­ 'exported energy' and considered in Module D.
and wind exposure, therefore designed to
building orientation, withstand outdoor conditions
Module C4
shading, temperature throughout their service life.
Not relevant according to the assumed end­of­life scenario.
Indoor environment (for
The declared products are
indoor applications), e.g. not intended for installation ­ Module D
temperature, moisture, inside a building. Module D contains the benefits and loads beyond the system
chemical exposure boundary related to the recycling of metals, which result from
Usage conditions, e.g. Standard use in any type of the treatment of recycled materials from the point of end­of­
frequency of use, building, i.e., opening/closing ­ waste status to the point of substitution (as loads) and the
mechanical exposure as often as necessary. substitution of primary resources (as benefits).
The declared products are It also includes the benefits and loads related to the energy
Maintenance e.g. required designed for a reference recovery from wooden plastic wastes in a municipal waste
frequency, type and quality service life of 30 years. They incineration plant as modelled in Module C3.
­
and replacement of are maintained by cleaning Only net flows leaving the product system are considered in
components water at the discretion of the module D.
building occupants.
5 Environmental Product Declaration ­ VELUX Group ­ VELUX Commercial continuous rooflights (PC­lysband)
5. LCA: Results
The set of characterisation factors EF 3.1 has been used.
DESCRIPTION OF THE SYSTEM BOUNDARY (X = INCLUDED IN LCA; MND = MODULE OR INDICATOR NOT DECLARED; MNR
= MODULE NOT RELEVANT)
Benefits and
Construction loads beyond
Product stage Use stage End of life stage
process stage the system
boundaries
la ire ta m w a Ry lp p u s tro p s n a rT g n iru tc a fu n a M e h t m o rf tro p s n a rTe tis e h t o t e ta g y lb m e s s A e s U e c n a n e tn ia M ria p e R tn e m e c a lp e R tn e m h s ib ru fe R y g re n e la n o ita re p Oe s u re ta w la n o ita re p Oe s u n o itc u rts n o c ­e Dn o itilo m e d tro p s n a rT g n is s e c o rp e ts a W la s o p s iD ­e s u e R­y re v o c e R­g n ilc y c e Rla itn e to p
A1 A2 A3 A4 A5 B1 B2 B3 B4 B5 B6 B7 C1 C2 C3 C4 D
X X X MND MND MND MND MNR MNR MNR MND MND X X X X X
RESULTS OF THE LCA - ENVIRONMENTAL IMPACT according to EN 15804+A2: 1 m² of VELUX Commercial continuous
rooflights
Parameter Unit A1-A3 C1 C2 C3 C4 D
Global Warming Potential total (GWP­total) kg CO 2 eq 1.32E+02 0 3.64E­01 3.86E+01 0 ­1.34E+02
Global Warming Potential fossil fuels (GWP­fossil) kg CO 2 eq 1.54E+02 0 3.64E­01 1.63E+01 0 ­1.3E+02
Global Warming Potential biogenic (GWP­biogenic) kg CO 2 eq ­2.18E+01 0 3.05E­04 2.24E+01 0 ­3.87E+00
Global Warming Potential luluc (GWP­luluc) kg CO 2 eq 3.5E­01 0 1.78E­04 1.1E­03 0 ­3.76E­01
Depletion potential of the stratospheric ozone layer (ODP) kg CFC11 eq 4.25E­06 0 7.98E­09 1.08E­07 0 ­1.57E­06
Acidification potential of land and water (AP) mol H+ eq 9.25E­01 0 1.7E­03 2.01E­02 0 ­6.28E­01
Eutrophication potential aquatic freshwater (EP­freshwater) kg P eq 5.4E­03 0 2.99E­06 7.5E­05 0 ­9E­03
Eutrophication potential aquatic marine (EP­marine) kg N eq 1.69E­01 0 6.69E­04 9E­03 0 ­9.86E­02
Eutrophication potential terrestrial (EP­terrestrial) mol N eq 1.88E+00 0 7.22E­03 9.95E­02 0 ­1.11E+00
Formation potential of tropospheric ozone photochemical oxidants kg NMVOC
6.69E­01 0 2.52E­03 2.81E­02 0 ­3.5E­01
(POCP) eq
Abiotic depletion potential for non fossil resources (ADPE) kg Sb eq 6.15E­04 0 1.13E­06 2.79E­06 0 3.01E­04
Abiotic depletion potential for fossil resources (ADPF) MJ 2.08E+03 0 5.25E+00 2.56E+01 0 ­1.48E+03
m3 world eq
Water use (WDP) 4.41E+01 0 2.29E­02 2.34E­01 0 ­1.26E+01
deprived
RESULTS OF THE LCA - INDICATORS TO DESCRIBE RESOURCE USE according to EN 15804+A2: 1 m² of VELUX Commercial
continuous rooflights
Parameter Unit A1-A3 C1 C2 C3 C4 D
Renewable primary energy as energy carrier (PERE) MJ 3.6E+02 0 8.18E­02 2.67E+02 0 ­2.18E+02
Renewable primary energy resources as material utilization
MJ 2.65E+02 0 0 ­2.65E+02 0 0
(PERM)
Total use of renewable primary energy resources (PERT) MJ 6.25E+02 0 8.18E­02 1.56E+00 0 ­2.18E+02
Non renewable primary energy as energy carrier (PENRE) MJ 1.89E+03 0 5.26E+00 2.18E+02 0 ­1.49E+03
Non renewable primary energy as material utilization (PENRM) MJ 1.92E+02 0 0 ­1.92E+02 0 0
Total use of non renewable primary energy resources (PENRT) MJ 2.08E+03 0 5.26E+00 2.57E+01 0 ­1.49E+03
Use of secondary material (SM) kg 1.98E+00 0 0 0 0 4.61E+00
Use of renewable secondary fuels (RSF) MJ 0 0 0 0 0 0
Use of non renewable secondary fuels (NRSF) MJ 0 0 0 0 0 0
Use of net fresh water (FW) m3 3.32E+00 0 1.42E­03 2.33E­02 0 ­8.63E­01
RESULTS OF THE LCA – WASTE CATEGORIES AND OUTPUT FLOWS according to EN 15804+A2:
1 m² of VELUX Commercial continuous rooflights
Parameter Unit A1-A3 C1 C2 C3 C4 D
Hazardous waste disposed (HWD) kg 2.25E­02 0 3.31E­05 1.34E­04 0 9.03E­03
Non hazardous waste disposed (NHWD) kg 3.91E+01 0 3.34E­01 4.81E­01 0 ­2.23E+01
Radioactive waste disposed (RWD) kg 4.72E­03 0 3.08E­06 6.32E­05 0 ­5.57E­03
Components for re­use (CRU) kg 0 0 0 0 0 0
Materials for recycling (MFR) kg 2.74E­01 0 0 6.31E+00 0 6.31E+00
Materials for energy recovery (MER) kg 0 0 0 0 0 0
Exported electrical energy (EEE) MJ 1.63E+00 0 0 8.21E+01 0 0
Exported thermal energy (EET) MJ 2.81E+00 0 0 1.41E+02 0 0
RESULTS OF THE LCA – additional impact categories according to EN 15804+A2-optional:
1 m² of VELUX Commercial continuous rooflights
Parameter Unit A1-A3 C1 C2 C3 C4 D
Disease
Incidence of disease due to PM emissions (PM) 1.19E­05 0 3.57E­08 3.76E­07 0 ­7.34E­06
incidence
Human exposure efficiency relative to U235 (IR) kBq U235 eq 3.3E+00 0 2.72E­03 3.39E­02 0 ­2.59E+00
6 Environmental Product Declaration ­ VELUX Group ­ VELUX Commercial continuous rooflights (PC­lysband)
Comparative toxic unit for ecosystems (ETP­fw) CTUe 1.97E+03 0 2.59E+00 4.44E+01 0 ­3.45E+02
Comparative toxic unit for humans (carcinogenic) (HTP­c) CTUh 2.46E­07 0 1.96E­10 7.59E­09 0 ­1.01E­07
Comparative toxic unit for humans (noncarcinogenic) (HTP­nc) CTUh 2.56E­06 0 4.07E­09 3.26E­08 0 ­1.24E­06
Soil quality index (SQP) SQP 2.91E+03 0 3.95E+00 3.04E+00 0 ­2.12E+02
Disclaimer 1 – for the indicator “Potential Human exposure efficiency relative to U235”. This impact category deals mainly with the
eventual impact of low­dose ionizing radiation on human health of the nuclear fuel cycle. It does not consider effects due to possible
nuclear accidents, occupational exposure or radioactive waste disposal in underground facilities. Potential ionizing radiation from the
soil, radon and from some construction materials is also not measured by this indicator.
Disclaimer 2 – for the indicators “abiotic depletion potential for non­fossil resources”, “abiotic depletion potential for fossil resources”,
“water (user) deprivation potential, deprivation­weighted water consumption”, “potential comparative toxic unit for ecosystems”,
“potential comparative toxic unit for humans – cancerogenic”, “Potential comparative toxic unit for humans ­ not cancerogenic”,
“potential soil quality index”. The results of this environmental impact indicator shall be used with care as the uncertainties on these
results are high as there is limited experience with the indicator.
6. LCA: Interpretation
Figure 1 illustrates the relative contributions of the different rooflights.
modules along the life cycle for VELUX Commercial continuous
product life cycle, except for the ADPelements (modules A1­
Figure 1: Relative environmental impacts of the different C4). The net positive impact ('load') of the ADPelements is
life cycle stages for VELUX Commercial continuous related to copper input as the copper cathode for the remelting
rooflights (modules A1–A3 = 100 %) of recycled aluminium.
By far the largest part of environmental impacts is caused The use of renewable primary energy is caused on the one
during production (modules A1­A3) of the VELUX Commercial hand by the share of renewable energy in the electricity mix
continuous rooflights (longlight), vaulted. The contributions of and on the other hand by the primary energy content of sawn
other life cycle stages are comparably small. timber and plywood used in the upstand; the production stage
is the main driver of this impact category whereas the
Benefits and burdens beyond the system boundary (module D) renewable energy stored in the wooden material is rebooked as
are in the order of ­164 % to ­28 % of the impacts over the used as an energy carrier in module C3.
7 Environmental Product Declaration ­ VELUX Group ­ VELUX Commercial continuous rooflights (PC­lysband)
are mainly caused by the European electricity mix used during
The use of non­renewable primary energy is mainly caused on the use phase.
the one hand by the share of non­renewable energy in the
electricity mix and heat consumption during production and on The LCA for the VELUX Commercial products have been
the other hand by the primary energy content of the plastic calculated for representative products, which are in fact quite
materials (polycarbonate); the production stage is the main close to the composition of the weighted average production in
driver of this impact category whereas the non­renewable 2022. To assess the possible variance, a 'maximum' version in
energy stored in the plastic components is rebooked as used terms of material intensity (highest upstand, highest number of
as an energy carrier in module C3. acrylic/polycarbonate layers, etc.) has been assessed per
product group. The higher material intensity of the maximum
Non­hazardous waste as the quantitatively most relevant waste version is more than compensated by a higher surface area
flows is mainly caused during maintenance due to the covered but lead to lower impact of around 10 % in most impact
replacement of the motor; hazardous and radio­active waste indicators.
7. Requisite evidence
7.1 Formaldehyde Not applicable; no test defined in applicable product standards.
No test defined in applicable product standards.
7.4 Fire gas toxicity
7.2 MDI No test defined in applicable product standards.
No test defined in applicable product standards.
7.5 VOC emissions
7.3 Checking for pretreatment of the substances used No test defined in applicable product standards.
8. References
Product category rules of IBU and procedures.
IBU (2021) ISO 14044
IBU (2021): General Instructions for the EPD Programme of the DIN EN ISO 14044:2006­07, Environmental management ­ Life
Institut Bauen und Umwelt e.V. Version 2.0, Institut Bauen und cycle assessment ­ Requirements and guidance.
Umwelt, Berlin.
ECHA candidate list
IBU (2021) The candidate list of substances of very high concern,
IBU (2021): PCR Part A: Calculation rules for the life cycle European Chemicals Agency, Helsinki. Available at:
assessment and requirements on the project report according https://echa.europa.eu/nl/­/four­newsubstances­added­to­the
to EN 15804+A2. Version 1.3, Institut Bauen und Umwelt e.V., candidate­list.
Berlin.
Regulation on biocidal products
IBU (2023) REGULATION (EU) No 528/2012 OF THE EUROPEAN
IBU (2023): PCR Part B: Requirements on the EPD for PARLIAMENT AND OF THE COUNCIL of 22 May 2012
windows and doors. Version 2023/04, Institut Bauen und concerning the making available on the market and use of
Umwelt e.V., Berlin. biocidal products.
Standards and legal documents Regulation (EU) Nr. 305/2011(CPR)
REGULATION (EU) No 305/2011 OF THE EUROPEAN
EN 14963 PARLIAMENT AND OF THE COUNCIL of 9 March 2011 laying
EN 14963:2006, Roof coverings ­ Continuous rooflights of down harmonised conditions for the marketing of construction
plastics with or without upstands ­ Classification, requirements products and repealing Council Directive 89/106/EEC.
and test methods.
COUNCIL REGULATION (EU) No 333/2011
EN 15804 COUNCIL REGULATION (EU) No 333/2011 of 31 March 2011
DIN EN 15804+A2:2022­03, sustainability of construction establishing criteria determining when certain types of scrap
works ­ Environmental product declarations ­ Core rules for the metal cease to be waste under Directive 2008/98/EC of the
product category construction products; German version EN European Parliament and of the Council.
15804: 2012+A2:2019 + AC:2021.
European Waste List (Waste index)
EN 16485 http://www.gesetze­im­internet.de/avv/anlage.htmEN 16485
DIN EN 16485:2014­07, Round and sawn timber ­
Environmental Product Declarations ­ Product category rules Additional references
for wood and wood­based products for use in construction;
German version EN 16485:2014. CEWEP Energy Report III
Reimann D.O. (2013): CEWEP Energy Report III (Status 2007
ISO 9001 – 2010); Results of Specific Data for Energy, R1 Plant
DIN EN ISO 9001:2015, Quality management systems ­ Efficiency Factor and NCV of 314 European Waste­to­Energy
Requirements. (WtE) Plants. CEWEP, Würzburg/Brussels, 2013.
ISO 14025 ecoinvent v3.9.1
DIN EN ISO 14025:2006­07, Environmental labels and ecoinvent v3.9.1, LCA database, 12/2022. Ecoinvent centre,
declarations ­ Type III Environmental declarations ­ Principles Zürich.
8 Environmental Product Declaration ­ VELUX Group ­ VELUX Commercial continuous rooflights (PC­lysband)
Publisher
Institut Bauen und Umwelt e.V. +49 (0)30 3087748­ 0
Hegelplatz 1 info@ibu­epd.com
10117 Berlin www.ibu­epd.com
Germany
Programme holder
Institut Bauen und Umwelt e.V. +49 (0)30 3087748­ 0
Hegelplatz 1 info@ibu­epd.com
10117 Berlin www.ibu­epd.com
Germany
Author of the Life Cycle Assessment
Dr. Frank Werner ­ Umwelt & Entwicklung + 41 (0)44 241 39 06
Kammelenbergstrasse 30 frank@frankwerner.ch
9011 St. Gallen http://www.frankwerner.ch/
Switzerland
Owner of the Declaration
VELUX Group +4545164871
Ådalsvej 99 birthe.kjeldsen@velux.com
2970 Hørsholm www.velux.com
Denmark
9 Environmental Product Declaration ­ VELUX Group ­ VELUX Commercial continuous rooflights (PC­lysband)
