ENVIRONMENTAL PRODUCT DECLARATION
as per ISO 14025 and EN 15804+A2
Owner of the Declaration dormakaba International Holding GmbH
Publisher Institut Bauen und Umwelt e.V. (IBU)
Programme holder Institut Bauen und Umwelt e.V. (IBU)
Declaration number EPD-DOR-20240263-CBA1-EN
Issue date 29.11.2024
Valid to 28.11.2029
Solenoid Locks SVx 6000
dormakaba
www.ibu-epd.com | https://epd-online.com
General Information
dormakaba Solenoid Locks SVx 6000
Programme holder Owner of the declaration
IBU – Institut Bauen und Umwelt e.V. dormakaba International Holding GmbH
Hegelplatz 1 DORMA Platz 1
10117 Berlin 58256 Ennepetal
Germany Germany
Declaration number Declared product / declared unit
EPD-DOR-20240263-CBA1-EN 1 piece of the product: Solenoid Lock SVx 6000, consisting of the following
items:
• Solenoid lock
• Product packaging
This declaration is based on the product category rules: Scope:
Building Hardware products, 01.08.2021 This Environmental Product Declaration refers to a specific solenoid lock
(PCR checked and approved by the SVR) (SVA 6000) manufactured by dormakaba. This EPD is also representing
the variants of SVP 6000 locks. The production site is located in Ennepetal
(Germany). Green electricity is being used at this production site.
Issue date
The data represents the year 2022.
29.11.2024
The owner of the declaration shall be liable for the underlying information
and evidence; the IBU shall not be liable with respect to manufacturer
information, life cycle assessment data and evidences.
Valid to
28.11.2029 The EPD was created according to the specifications of EN 15804+A2. In
the following, the standard will be simplified as EN 15804.
Verification
The standard EN 15804 serves as the core PCR
Independent verification of the declaration and data according to ISO
14025:2011
internally X externally
Dipl.-Ing. Hans Peters
(Chairman of Institut Bauen und Umwelt e.V.)
Florian Pronold Matthias Klingler,
(Managing Director Institut Bauen und Umwelt e.V.) (Independent verifier)
1 Environmental Product Declaration - dormakaba - Solenoid Locks SVx 6000
Product
The solenoid locks have following technical properties:
Product description/Product definition
Self-locking emergency escape locks automatically lock doors
Name Value Unit
after each closing whether mechanically or motor-controlled.
V DC
The emergency escape function allows the door to be opened Supply voltage 12 or 24
stabilized
at any time in the exit direction by simply operating the lever
handle. Mechanical opening from the outside remains possible Temperature range - 25 to °C
at any time by unlocking the profile cylinder insert. +70
Relative humidity up to 95% at 55 °C
SVP 6000 microswitch-monitored emergency-escape lock with Protection category 54 IP
automatic locking action and with divided follower, mechanical Rear backset 33 mm
sequential control and signalling through integrated monitoring
Distance between door handle and
contact, automatically locks the doors after each closing cycle. 72 mm
locking cylinder (for profile cylinder)
The automatic deadbolt throw of 20 mm ensures that the door
Distance between door handle and
is always locked in accordance with property insurance 74 mm
locking cylinder (for round cylinder)
requirements. Meanwhile, thanks to the added one-sided
emergency escape function, the door can be opened at any Bolt throw 20 mm
time in the exit direction by simply operating the lever handle or
Performance data of the product with respect to its
it can be opened from the outside through a key or engageable
characteristics in accordance with the relevant technical
external lever.
provision which can be applied are mentioned above.
SVP 6000 Base materials/Ancillary materials
• An electrically-monitored panic lock with a split follower The major material composition including the packaging of the
for the electrical engagement/disengagement product is listed below:
the outside handle and manipulation-protected detectors Name Value Unit
Steel 66 %
SVA 6000
Stainless steel 16 %
• Electrically monitored emergency-escape lock with split Paper 15 %
follower for the electrical engagement/
Plastics 2 %
disengagement of the outside lever handle
Electronics 1 %
• Status message for trip latch, bolt, cylinder locking and
lever handle The products include partial articles which contain substances
listed in the Candidate List of REACH Regulation
1907/2006/EC (date: 23.01.2024) exceeding 0.1 percentage by
For the use and application of the product the respective mass: yes
national provisions at the place of use apply. The standards
• Lead (Pb): 7439-92-1 (CAS-No.) is included in some of
which can be applied are the following:
the alloys used. The concentration of lead in each
• EN 179 individual alloy does not exceed 4.0% (by mass).
• EN 1125
• EN 12209 The Candidate List can be found on the ECHA website
• EN 14846 address: https://echa.europa.eu/de/home.
• Restriction of Hazardous Substances (RoHS)
Reference service life
The reference service life of the Solenoid Locks SVx 6000
Application series amounts to 20 years and depends on the application and
Solenoid locks are suitable for use in emergency exits and frequency of use. For repairs or renewals, suitable spare parts
escape routes in compliance with EN 179 or on panic doors are available. The locks are tested and certified to EN 14846,
with a horizontal push bar in compliance with EN 1125. meaning they are designed to withstand a minimum of 200.000
cycles.
Technical Data
LCA: Calculation rules
The type of EPD is according to EN 15804: "cradle to gate with
Declared Unit options, modules C1–C4, and module D". The following
The declared unit is 1 piece of the product including packaging: modules are declared:
SVx 6000. A1-A3, B6, C1-C4, D and additional modules: A4 + A5
Name Value Unit
Declared unit 1 piece/product Production - Module A1-A3
The product stage includes:
Mass of the declared product without
0.99 kg — A1, raw material extraction, processing and mechanical
packaging
treatments, processing
Mass of packaging 0,05
of secondary material input (e.g. recycling processes),
— A2, transport to the manufacturer,
— A3, manufacturing and assembly including provision of all
System boundary materials, products and energy,
2 Environmental Product Declaration - dormakaba - Solenoid Locks SVx 6000
as well as waste processing up to the end-of waste state. — C4, disposal; including provision and all transport, provision
of all materials, products
Construction stage - Modules A4-A5 and related energy and water use.
The construction process stage includes: Module D (Benefits and loads beyond the system boundary)
— A4, transport to the building site; includes:
— A5, installation into the building; including provision of all — D, recycling potentials, expressed as net impacts and
materials, products and energy, benefits.
as well as waste processing up to the end-of waste state or
disposal of final residues during Geographic Representativeness
the construction process stage. Land or region, in which the declared product system is
manufactured, used or handled at the end of the product´s
Use stage - Module B6 lifespan: Global
The use stage related to the operation of the building includes:
— B6, operational energy use
Comparability
Basically, a comparison or an evaluation of EPD data is only
End-of-life stage– Modules C1-C4 and D
possible if all the data sets to be compared were created
The end-of-life stage includes:
according to EN 15804 and the building context, respectively
— C1, de-construction, demolition:
the product-specific characteristics of performance, are taken
— C2, transport to waste processing;
into account. GaBi, SP40.
— C3, waste processing for reuse, recovery and/or recycling;
LCA: Scenarios and additional technical information
Operational energy use (B6)
Characteristic product properties of biogenic carbon
Note: 1 kg of biogenic carbon is equivalent to 44/12 kg of CO2 Name Value Unit
Name ValueUnit Energy consumption for 1 year 7.59 kWh
kg Active state (hours/day) 0.25 hrs
Biogenic carbon content in product 0.04
C Idle state (hours/day) 23.75 hrs
Biogenic carbon content in accompanying kg Electrical power active state 2.88 W
0.02
packaging C Electrical power in idle state 1.2 W
Note: 1 kg of biogenic carbon is equivalent to 44/12 kg of CO .
2 End of life (C1-C4)
C1: The product dismantling from the building is done manually
without environmental burden.
C2: Transport to waste management is 50 km.
Name Value Unit
Transport to the building site (A4)
Collected separately waste type 0.99 kg
Name Value Unit
Recycling 0.97 kg
Litres of fuel (per 1kg) 0.00276 l/100km
Energy recovery 0.02 kg
Transport distance via truck (for scaling) 100 km
The product is disassembled in a recycling process. Material
Capacity utilisation (including empty runs) 55 %
recycling is then assumed for the metals. The plastic
Transport distance via ship 15000 km
components are assumed to be incinerated with energy
The product is transported via truck. The product is stored in recovery.
the dormakaba logistic centre in Germany. The main Region for the End of Life is: Europe.
distribution region is Europe and Asia. In order to allow scaling
to a specific point of installation 100 km are declared as well.
Reuse, recovery and/or recycling potentials (D), relevant
scenario information
Installation into the building (A5) Name Value Unit
Name Value Unit Recycling 100 %
Waste packaging (paper) 0.045 kg
The collection rate is 100 %.
Reference service life
Name Value Unit
Life Span according to the manufacturer 20 a
3 Environmental Product Declaration - dormakaba - Solenoid Locks SVx 6000
LCA: Results
DESCRIPTION OF THE SYSTEM BOUNDARY (X = INCLUDED IN LCA; MND = MODULE OR INDICATOR NOT DECLARED; MNR
= MODULE NOT RELEVANT)
Benefits and
Construction loads beyond
Product stage Use stage End of life stage
process stage the system
boundaries
la ire ta m w a Ry lp p u s tro p s n a rT g n iru tc a fu n a M e h t m o rf tro p s n a rTe tis e h t o t e ta g y lb m e s s A e s U e c n a n e tn ia M ria p e R tn e m e c a lp e R tn e m h s ib ru fe R y g re n e la n o ita re p Oe s u re ta w la n o ita re p Oe s u n o itc u rts n o c -e Dn o itilo m e d tro p s n a rT g n is s e c o rp e ts a W la s o p s iD -e s u e R-y re v o c e R-g n ilc y c e Rla itn e to p
A1 A2 A3 A4 A5 B1 B2 B3 B4 B5 B6 B7 C1 C2 C3 C4 D
X X X X X MND MND MNR MNR MNR X MND X X X X X
RESULTS OF THE LCA - ENVIRONMENTAL IMPACT according to EN 15804+A2: 1 piece Solenoid Lock SVX 6000
Parameter Unit A1-A3 A4 A5 B6 C1 C2 C3 C4 D
GWP-total kg CO 2 eq 6.76E+00 9E-03 6.5E-02 6.14E+01 0 4E-03 2.33E-01 0 -2.29E+00
GWP-fossil kg CO 2 eq 6.98E+00 9E-03 2E-03 6.11E+01 0 4E-03 5.2E-02 0 -2.29E+00
GWP-biogenic kg CO 2 eq -2.22E-01 4E-04 6.3E-02 2.04E-01 0 1.79E-04 1.81E-01 0 2E-03
GWP-luluc kg CO 2 eq 5.34E-03 2.06E-07 1.06E-06 8.9E-02 0 9.21E-08 4.55E-06 0 -2E-03
ODP kg CFC11 eq 7.47E-11 9.14E-19 1.16E-17 1.34E-12 0 4.08E-19 4.72E-17 0 -1.41E-15
AP mol H+ eq 4.26E-02 8.67E-06 1.81E-05 1.35E-01 0 3.87E-06 3.51E-05 0 -1.9E-02
EP-freshwater kg P eq 1.67E-05 1.85E-09 2.27E-09 1.63E-04 0 8.28E-10 7.29E-09 0 -9.89E-07
EP-marine kg N eq 6.16E-03 2.76E-06 6.52E-06 3E-02 0 1.23E-06 1.05E-05 0 -3E-03
EP-terrestrial mol N eq 6.71E-02 3.07E-05 8.13E-05 3.15E-01 0 1.37E-05 1.64E-04 0 -2.7E-02
kg NMVOC
POCP 1.84E-02 7.8E-06 1.73E-05 8.2E-02 0 3.48E-06 2.87E-05 0 -8E-03
eq
ADPE kg Sb eq 6.98E-04 2.6E-10 1.84E-10 1.77E-05 0 1.16E-10 6.97E-10 0 -6.82E-04
ADPF MJ 9.21E+01 1.23E-01 2E-02 1.07E+03 0 5.5E-02 6.2E-02 0 -2.37E+01
m3 world eq
WDP 1.17E+00 1.7E-05 8E-03 1.33E+01 0 7.58E-06 2.4E-02 0 -3.96E-01
deprived
GWP = Global warming potential; ODP = Depletion potential of the stratospheric ozone layer; AP = Acidification potential of land and water; EP =
Eutrophication potential; POCP = Formation potential of tropospheric ozone photochemical oxidants; ADPE = Abiotic depletion potential for non-fossil
resources; ADPF = Abiotic depletion potential for fossil resources; WDP = Water (user) deprivation potential)
RESULTS OF THE LCA - INDICATORS TO DESCRIBE RESOURCE USE according to EN 15804+A2: 1 piece Solenoid Lock SVX
6000
Parameter Unit A1-A3 A4 A5 B6 C1 C2 C3 C4 D
PERE MJ 2.04E+01 3.87E-04 5.5E-01 4.76E+02 0 1.73E-04 1.23E+00 0 -2.14E+00
PERM MJ 1.76E+00 0 -5.46E-01 0 0 0 -1.21E+00 0 0
PERT MJ 2.22E+01 3.87E-04 4E-03 4.76E+02 0 1.73E-04 1.3E-02 0 -2.14E+00
PENRE MJ 9.21E+01 1.23E-01 2E-02 1.07E+03 0 5.5E-02 6.79E-01 0 -2.38E+01
PENRM MJ 6.17E-01 0 0 0 0 0 -6.17E-01 0 0
PENRT MJ 9.27E+01 1.23E-01 2E-02 1.07E+03 0 5.5E-02 6.2E-02 0 -2.38E+01
SM kg 3.98E-01 0 0 0 0 0 0 0 0
RSF MJ 0 0 0 0 0 0 0 0 0
NRSF MJ 0 0 0 0 0 0 0 0 0
FW m3 4.1E-02 6.95E-07 1.88E-04 5.51E-01 0 3.1E-07 5.66E-04 0 -1.5E-02
PERE = Use of renewable primary energy excluding renewable primary energy resources used as raw materials; PERM = Use of renewable primary
energy resources used as raw materials; PERT = Total use of renewable primary energy resources; PENRE = Use of non-renewable primary energy
excluding non-renewable primary energy resources used as raw materials; PENRM = Use of non-renewable primary energy resources used as raw
materials; PENRT = Total use of non-renewable primary energy resources; SM = Use of secondary material; RSF = Use of renewable secondary fuels;
NRSF = Use of non-renewable secondary fuels; FW = Use of net fresh water
RESULTS OF THE LCA – WASTE CATEGORIES AND OUTPUT FLOWS according to EN 15804+A2:
1 piece Solenoid Lock SVX 6000
Parameter Unit A1-A3 A4 A5 B6 C1 C2 C3 C4 D
HWD kg 7.36E-07 1.19E-11 3E-11 4.45E-07 0 5.33E-12 1.15E-10 0 -6.57E-08
NHWD kg 1.97E-01 1.26E-05 2E-03 7.62E-01 0 5.61E-06 6E-03 0 -8.7E-02
RWD kg 3.4E-03 1.32E-07 1.07E-06 1.63E-01 0 5.89E-08 3.11E-06 0 -2.23E-04
CRU kg 0 0 0 0 0 0 0 0 0
MFR kg 0 0 0 0 0 0 8.05E-01 0 0
MER kg 0 0 0 0 0 0 0 0 0
EEE MJ 0 0 9.8E-02 0 0 0 3.64E-01 0 0
EET MJ 0 0 1.77E-01 0 0 0 7.03E-01 0 0
4 Environmental Product Declaration - dormakaba - Solenoid Locks SVx 6000
HWD = Hazardous waste disposed; NHWD = Non-hazardous waste disposed; RWD = Radioactive waste disposed; CRU = Components for re-use;
MFR = Materials for recycling; MER = Materials for energy recovery; EEE = Exported electrical energy; EET = Exported thermal energy
RESULTS OF THE LCA – additional impact categories according to EN 15804+A2-optional:
1 piece Solenoid Lock SVX 6000
Parameter Unit A1-A3 A4 A5 B6 C1 C2 C3 C4 D
Disease
PM 4.63E-07 4.56E-11 1E-10 1.13E-06 0 2.04E-11 2.45E-10 0 -1.98E-07
incidence
IR kBq U235 eq 3.5E-01 1.89E-05 1.66E-04 2.67E+01 0 8.42E-06 4.33E-04 0 -2.8E-02
ETP-fw CTUe 4.77E+01 8.7E-02 1E-02 4.6E+02 0 3.9E-02 2.6E-02 0 -7.21E+00
HTP-c CTUh 2.14E-07 1.64E-12 5.11E-13 1.27E-08 0 7.31E-13 1.88E-12 0 -2.51E-09
HTP-nc CTUh 1.09E-07 7E-11 2.22E-11 4.68E-07 0 3.13E-11 1.15E-10 0 -1.43E-08
SQP SQP 4.68E+01 3.16E-04 5E-03 3.42E+02 0 1.41E-04 1.8E-02 0 -1.64E+00
PM = Potential incidence of disease due to PM emissions; IR = Potential Human exposure efficiency relative to U235; ETP-fw = Potential comparative
Toxic Unit for ecosystems; HTP-c = Potential comparative Toxic Unit for humans (cancerogenic); HTP-nc = Potential comparative Toxic Unit for humans
(not cancerogenic); SQP = Potential soil quality index
Disclaimer 1 – for the indicator “Potential Human exposure efficiency relative to U235”. This impact category deals mainly with the
eventual impact of low-dose ionizing radiation on human health of the nuclear fuel cycle. It does not consider effects due to possible
nuclear accidents, occupational exposure or radioactive waste disposal in underground facilities. Potential ionizing radiation from the
soil, radon and from some construction materials is also not measured by this indicator.
Disclaimer 2 – for the indicators “abiotic depletion potential for non-fossil resources”, “abiotic depletion potential for fossil resources”,
“water (user) deprivation potential, deprivation-weighted water consumption”, “potential comparative toxic unit for ecosystems”,
“potential comparative toxic unit for humans – cancerogenic”, “Potential comparative toxic unit for humans - not cancerogenic”,
“potential soil quality index”. The results of this environmental impact indicator shall be used with care as the uncertainties on these
results are high as there is limited experience with the indicator.
This EPD was created using a software tool.
References
Directive 2011/65/EU of the European Parliament and of the
EN 179 Council of 8 June 2011 on the restriction of the use of certain
EN 179:2008-04; Building hardware - Emergency exit devices hazardous substances in electrical and electronic equipment
operated by a lever handle or push pad, for use on escape
routes - Requirements and test methods Further References
EN 1125 IBU 2021
EN 1125;2008-04; Building hardware - Panic exit devices General Instructions for the EPD programme of Institut Bauen
operated by a horizontal bar, for use on escape routes - und Umwelt e.V. Version 2.0, Berlin: Institut Bauen und Umwelt
Requirements and test methods e.V., 2021. www.ibu-epd.com
EN 12209 GaBi
EN 12209:2016-10; Building hardware - Mechanically operated Sphera Solutions GmbH Gabi Software System and Database
locks and locking plates - Requirements and test methods for Life Cycle Engineering 1992-2020 Version 10.0.0.71
University of Stuttgart Leinfelden-Echterdingen
EN 14846
EN 14846:2008-11; Building hardware - Locks and latches - GaBi ts documentation
Electromechanically operated locks and striking plates - GaBi life cycle inventory data documentation (https://www.gabi-
Requirements and test methods software.com/support/gabi/gabidatabase- 2020-lci-
documentation/)
EN 15804
EN15804+A2:2019+AC:2021; Sustainability of construction LCA-tool dormakaba
works — Environmental Product Declarations — Core rules for LCA tool DHW. LCA-Tool No.: IBU-DOR-202104-LT1-EN.
the product category of construction products Developed by Sphera Solutions GmbH
ISO 14025 PCR Part A
DIN EN ISO 14025:201110; Environmental labels and PCR – Part A: Calculation Rules for the Life Cycle Assessment
declarations — Type III environmental declarations — and Requirements on the Project Report according to EN
Principles and procedures 15804+A2:2019, Version 1.0, 2020, Institut Bauen und Umwelt
e.V., www.ibu-epd.com
REACH
Regulation (EC) No 1907/2006 of the European Parliament and PCR Part B
of the Council on the Registration, Evaluation, Authorisation PCR – Part B: Requirements on the EPD for Building Hardware
and Restriction of Chemicals (REACH) product, version 08/2021, Institut Bauen und Umwelt e.V.,
www.ibu-epd.com.
ROHS3 Directive
5 Environmental Product Declaration - dormakaba - Solenoid Locks SVx 6000
Publisher
Institut Bauen und Umwelt e.V. +49 (0)30 3087748- 0
Hegelplatz 1 info@ibu-epd.com
10117 Berlin www.ibu-epd.com
Germany
Programme holder
Institut Bauen und Umwelt e.V. +49 (0)30 3087748- 0
Hegelplatz 1 info@ibu-epd.com
10117 Berlin www.ibu-epd.com
Germany
Author of the Life Cycle Assessment
dormakaba International Holding GmbH +49 2333 793-0
DORMA Platz 1 info.de@dormakaba.com
58256 Ennepetal www.dormakaba.com
Germany
Owner of the Declaration
dormakaba International Holding GmbH +49 2333 793-0
DORMA Platz 1 info.de@dormakaba.com
58256 Ennepetal www.dormakaba.com
Germany
6 Environmental Product Declaration - dormakaba - Solenoid Locks SVx 6000
