ENVIRONMENTAL PRODUCT DECLARATION
as per ISO 14025 and EN 15804+A2
Owner of the Declaration Sonae Arauco, S.A.
Publisher Institut Bauen und Umwelt e.V. (IBU)
Programme holder Institut Bauen und Umwelt e.V. (IBU)
Declaration number EPD-SON-20230518-IBA1-EN
Issue date 10.01.2024
Valid to 09.01.2029
Medium density fibreboard (MDF), uncoated
Sonae Arauco, S.A.
www.ibu-epd.com | https://epd-online.com
1. General Information
Sonae Arauco, S.A. Medium density fibreboard (MDF), uncoated
Programme holder Owner of the declaration
IBU – Institut Bauen und Umwelt e.V. Sonae Arauco, S.A.
Hegelplatz 1 Calle Ulises 26­18
10117 Berlin 28043 Madrid
Germany Spain
Declaration number Declared product / declared unit
EPD­SON­20230518­IBA1­EN Medium density fiberboard, uncoated, per m3
This declaration is based on the product category rules: Scope:
Wood­based panels, 01.08.2021 This document refers to MDF manufactured in the following plants of the
(PCR checked and approved by the SVR) Sonae Arauco Group:
• Sonae Arauco Beeskow GmbH, Radinkendorfer Strasse 71,
15848 Beeskow, Germany
Issue date
• Soena Arauco Deutschland AG, Grecostr. 1, 49716 Meppen,
10.01.2024 Germany
• Sonae Arauco Portugal, SA, Água Levada Apartado 168, 3534­
956 Mangualde, Portugal
Valid to • Sonae Arauco South Africa (Pty) Ltd, Heidelberg Road, Rocky
Drift, White River, Republic of South Africa
09.01.2029
• Sonae Arauco, S.A., Calle de Los Titulos, 29, 47009 Valladolid,
Spain
The production volume of these plants covers 100 % of the total production
of MDF by Sonae Arauco group.
The owner of the declaration shall be liable for the underlying information
and evidence; the IBU shall not be liable with respect to manufacturer
information, life cycle assessment data and evidences.
The EPD was created according to the specifications of EN 15804+A2. In
the following, the standard will be simplified as EN 15804.
Verification
Dipl.­Ing. Hans Peters
(Chairman of Institut Bauen und Umwelt e.V.) The standard EN 15804 serves as the core PCR
Independent verification of the declaration and data according to ISO
14025:2011
internally X externally
Florian Pronold Mr Olivier Muller,
(Managing Director Institut Bauen und Umwelt e.V.) (Independent verifier)
1 Environmental Product Declaration ­ Sonae Arauco, S.A. ­ Medium density fibreboard (MDF), uncoated
2. Product
MDF ranging in thicknesses from 2 to 45 mm can be purchased
2.1 Product description/Product definition as uncoated boards. The boards are offered in standard
Medium density fibreboard (MDF) is a panel­shaped wood­ formats. Fixed formats are also available, and selected formats
based material in accordance with EN 316 that is manufactured are offered with a tongue and groove profile.
in a dry process by means of compression under heat of wood
fibres with adhesive. Uncoated MDF boards can be unsanded, The following values include minimum and maximum
sanded and/or profiled. dimensions for the boards supplied worldwide. Some of the
Due to their various densities and adhesive systems, they can combinations for sizes may not be available in all markets.
display a variety of material properties and qualities like
moisture resistance, fire retardant, load­bearing or others. Thickness 2 ­ 45 mm
For the placing on the market in the European Union/European Width 500 ­ 2850 mm
Free Trade Association (EU/EFTA) (with the exception of Length 1025 ­ 6250 mm
Switzerland), Regulation (EU) 305/2011 applies. When
applicable, the products need a Declaration of Performance For updated information on available dimensions, please refer
(DOP) taking into consideration EN 13986:2004+A1:2015 to:
Wood-based panels for use in construction - Characteristics, www.sonaearauco.com
evaluation of conformity and marking and the CE­marking.
For the application and use the respective national provisions 2.5 Base materials/Ancillary materials
apply. Raw MDF bonded with urea­formaldehyde/melamine­urea­
formaldehyde (UF/MUF) consist of (dimensions as % by mass):
2.2 Application
• Wood chips: approx. 80 %
The area of application for uncoated MDF primarily involves
• Water: 4 – 11%
decorative interior furnishings and furniture construction but
• UF glue / MUF glue (urea resin, melamine urea resin): 9
also interior construction such as trade fair stands and shop
% – 25%
design.
• Paraffin wax emulsion: 0.5 % – 3 %
Apart from an extensive basic range, special MDF variants are
Raw MDF bonded with polymeric diphenylmethane
also available, e.g. fire­retardant MDF as well as MDF with
diiscocyanate (PMDI) consist of (dimensions as % by mass):
increased resistance to moisture.
• Wood chips: approx. 90 %
2.3 Technical Data • Water: 4 – 8 %
Due to the large variability of product properties and quality • PMDI glue (polymer 4.4' diphenyl methane
grades, the table below only shows the range of technical diisocyanate): 3.5%
characteristics for standard boards. • Paraffin wax emulsion: 0.5 – 3%
Wood from indigenous, largely regional forest plantations is
Special boards as well as customized products have different used for manufacturing raw MDF. This wood is typically
technical characteristics from the ones shown. procured from forests within an average radius of 250 km of the
Name Value Unit plants' locations.
Furthermore, sawmill residues are also used as raw materials
Gross density according to EN 323 680 ­ 860 kg/m3
in the production of MDF.
Bending strength (longitudinal) according to
17 ­ 23 N/mm2
EN 310 The entire range can be made available on request as FSC®
E­module (longitudinal) according to EN 1900 ­ N/mm2 certified or PEFC (program for the endorsement of forest
310 2700 certification) certified products.
Tensile strength rectangular according to Additionally, the complete range includes CE­marked products.
0.5 ­ 0.9 N/mm2
EN 319
Thickness swelling according to EN 317 8 ­ 45 % This product contains substances listed in the ECHA candidate
list (date: 08.06.2021) exceeding 0.1 percentage by mass:
Moisture content according to EN 322 5 ­ 9
· no
Performance data of the product in accordance with the
declaration of performance with respect to its essential This product contains other carcinogenic, mutagenic, reprotoxic
characteristics according to: (CMR) substances in categories 1A or 1B which are not on the
EN 316, Wood fibre boards ECHA candidate list, exceeding 0.1 percentage by mass:
EN 622-1, Fibreboards · no
EN 622-5, Fibreboards
EN 13986 Wood-based panels for use in construction
ISO 16895-1, Wood-based panels Biocide products were added to this construction product or it
ISO 16895-2, Wood-based panels has been treated with biocide products (this then concerns a
treated product as defined by the (EU) Regulation on biocidal
Declaration of Performance (DoP) products No. 528/2012:
· no
For more details on technical information, please see the
respective products' Declaration of Performance (DoP) 2.6 Manufacture
available at: The manufacturing of MDF comprises the following steps:
www.sonaearauco.com
1. Debarking the logs
2. Chipping the wood to chips of approx. 3 x 3 cm in size
2.4 Delivery status
3. Boiling the chips
2 Environmental Product Declaration ­ Sonae Arauco, S.A. ­ Medium density fibreboard (MDF), uncoated
4. Defibring in the refiner 11. Stacking
5. Glueing the fibres with resin 12. Sanding the top or underside after the air­conditioning
6. Drying the fibres to a residual moisture content phase
7. Scattering the glued fibre on a forming belt
8. Pressing the fibre mat in a continuous hot press under high Leftovers incurred during board manufacture are typically
pressure redirected to be used as fuel to supply the energy needs of the
9. Cutting the continuous mat into raw board formats manufacturing process on site.
10. Cooling the raw boards in star coolers A process diagram is presented below.
system following pre­treatment. Sludges generated within the
water treatment can be used in agriculture as a fertiliser.
The production sites are certified according to the following
standards: Noise: Noise surveys are required and are performed for each
site according to respective national regulations. Noise­
• ISO 9001
intensive plant areas such as chipping are encapsulated or
• ISO 45001
protected appropriately by structural measures.
• ISO 50001:2011 (European sites).
2.7 Environment and health during manufacturing Whenever necessary (close to non­encapsulated areas), the
Health protection: Due to the manufacturing conditions, no use of ear protection is required (PPE, Personal Protective
special health protection measures over and beyond the Equipment) within Sonae Arauco sites, as an additional safety
regulatory guidelines are required. The reference occupational measure.
exposure limit values are complied with.
The production sites are all ISO 14001 certified.
Emissions into air: Waste air generated during production is
2.8 Product processing/Installation
cleaned in accordance with regulatory requirements. Emissions
Sonae Arauco MDF can be sawn, milled, planed, sanded and
have to comply with the values specified by the operation
drilled using standard machinery or (electric) power tools.
licenses of the different sites, specified according to national
Carbide­tipped tools should be given preference, especially on
laws.
circular saws. Respiratory protection should be worn when
using hand­held equipment without suction devices.
Emissions into water/soil: No normal process contamination
of water or soil exists. Waste water generated in the process is
Please refer to the respective devices' datasheets for further
treated onsite and/or directed into the municipal sewage
processing recommendations.
3 Environmental Product Declaration ­ Sonae Arauco, S.A. ­ Medium density fibreboard (MDF), uncoated
Fire
2.9 Packaging
Fire retardant classification is done according to EN 13986. Fire
Sonae Arauco MDF is supplied on squared timber bound by retardant classes are defined in accordance with EN 13501-1.
plastic or metal bands and covered with corrugated cardboard The fire classification of MDF with a raw density of ≥ 600 kg/m³
and, on the bottom, with a cover board. and a thickness ≥ 9 mm is D­s2, d0. The boards with lower
density or thickness are in class E.
MDF and steel or PET packing bands for transport packaging Fire retardant boards are classified as B­s1, d0 and B­s2, d0.
can be sorted and directed to the recycling circuits. If re­use or
Fire safety (for standard MDF boards)
recycling is impractical, the packaging should not be landfilled,
but rather directed towards energy recovery. Name Value
Packaging disposal information is available at: Building material class D/E
www.sonaearauco.com Smoke gas development S2
2.10 Condition of use Burning droplets d0
The components making up uncoated MDF correspond with the
base material compositions as outlined in Clause 2.6. During Water
hot pressing, the binding agent is linked irreversibly by means No ingredients are washed out which could be hazardous to
of poly­condensation and firmly bonded with the wood. The water. MDF is not resistant to permanent exposure to water.
binding agents are chemically and stably bound to the wood.
Mechanical destruction
VOC emissions: Sonae Arauco MDF is labelled as class A+, A Mechanical destruction of MDF boards can result in sharp
or B according to the French regulation on the labelling of edges on the broken panel edges (risk of injury).
emissions of volatile pollutants from construction and
decoration products (with reference to the wall scenario, as a 2.14 Re-use phase
worst case). Recycling: Sonae Arauco MDF from construction can be
collected separately and utilised in the manufacture of MDF or
Sonae Arauco MDF at an average density of 760 kg/m3 stores other types of wood­based boards. This is based on the
1140 kg CO equivalent over its service life. condition that the wooden boards are not fully glued.
2
2.11 Environment and health during use Energy recovery: Due to the high heating value of approx.
Environmental protection: According to current information, 16.5 MJ/kg at 20 % moisture content assumed for post­
water, air and soil are not exposed to any dangers when the consumer boards, MDF can be used for energy recovery and
respective products outlined above are used as designated. the generation of heat and electricity (e.g. in CHP plants),
following the cascading principle for wood.
Health protection: According to current information, no
2.15 Disposal
damage to or impairment of health can be anticipated when
Sonae Arauco MDF leftovers and residual materials incurred as
MDF is used as designated.
a result of demolition measures on the building sites should be
primarily directed towards material recycling. If this is not
With the exception of low volumes of formaldehyde for
possible, they must be directed toward energy recovery instead
UF/MUF­bonded MDF, VOC emissions from products are
of landfilling.
negligible, and are natural wood ingredients.
2.12 Reference service life Waste code according to the Regulation on the European
Due to the wide range of applications of Sonae Arauco MDF, no Waste List: 17 02 01
reference service life is declared.
2.16 Further information
Description of the influences on the ageing of the product when
Further information such as technical datasheets, etc. can be
applied in accordance with the rules of technology.
downloaded under:
2.13 Extraordinary effects www.sonaearauco.com
3. LCA: Calculation rules
Modules A1 – A3 of the production stage cover the
3.1 Declared Unit manufacturing of the products, including raw material extraction
The declared unit for the LCA is 1 m3 of average uncoated and processing, energy generation, the production of ancillary
Sonae Arauco medium density fibreboard. products and packaging materials, transport, as well as all
waste treatment processes. Eventual benefits of recycling or
Information on the declared unit
energy recovery are neglected.
Name Value Unit
The resource aspects of wood were inventoried via material
Declared unit 1 m3 inherent properties such as resource extraction of CO from the
2
Mass reference 760 kg/m3 atmosphere and the lower heating value as the use of
renewable energy. Material inherent properties are subject to
The weighted average was calculated based on production
co­product allocation as ruled in EN 15804.
volumes from the plants in all countries where Sonae Arauco
was operating in 2021 (some plants 2020).
Module A4 covers the transport of the product from the
3.2 System boundary production site to the construction site by a lorry over a default
Type of the EPD: cradle­to­gate with modules C1 to C4 and distance of 460 km.
module D (A1 – A3, C and D)
Module A5 covers the transport of the packaging material from
4 Environmental Product Declaration ­ Sonae Arauco, S.A. ­ Medium density fibreboard (MDF), uncoated
the construction site and its disposal. Default end­of­waste related to production processes but to the maintenance of
states for the packaging materials from the packed products at infrastructure, e.g. acetylene and oxygen for soldering, etc.
the construction site are defined in analogy for wastes With this approach mass and energy flows below 1 percent of
occurring in modules A1 – A3. Eventual further inputs for the total mass and energy flows caused by the declared products
installation of the products are not considered due to the broad were included in the assessment.
applicability of the assessed products. Beyond that, no material or energy flows were neglected that
The substituted primary material from the net amount of would have been known by the persons responsible for the
recycled material and from recovered energy exported from the project and that could have been expected to contribute
product system in Module A5 is declared in Module D. significantly to the environmental indicators declared. It can
thus be assumed that the total contribution of the neglected
Module C1 manual deconstruction is assumed. The declared processes is not higher than 5 % of the declared impact
values are thus 0. categories.
Module C2 includes the transport of the de­constructed product 3.5 Background data
to a recycling centre by over 50 km. Datasets from ecoinvent v3.8 (cut­off by classification) were
used as background data exclusively. Therefore, the latest
Module C3 covers the preparation of the post­consumer board update of the background data took place in 2021.
to become a secondary fuel; the end­of­waste status for
3.6 Data quality
recycled wood­based boards is defined as the point where they
have been sorted and chipped, ready to be used as secondary The requirements on the data quality and the background data
fuels. correspond to the provisions in EN 15804:
In line with EN 16485, the export of the biogenic carbon stored • Data are as current as possible. Datasets used for
in the board, expressed in CO ­equivalent is also reported in calculations were updated within the last 10 years for
2
module C3. generic data and within the last 5 years for producer­
specific data;
Module C4 is not relevant for the assumed end­of­life scenario. • Datasets are based on 1­year averaged data as a
The declared values are thus 0. general rule;
• The time period over which inputs to and outputs from
Module D compiles all the benefits and burdens associated with the system are accounted for is 100 years from the year
the secondary fuels, secondary materials and exported energy for which the data set is deemed representative;
leaving the production system in the modules A5 and C3. • The technological coverage reflects the physical reality
Therefore, module D covers the avoided burdens from recycling of the declared products;
and from energy recovered from the waste treatment in module • The background datasets comply with the quality
A5 as well as the transport of the obsolete boards to a biomass guidelines of ecoinvent v.3; deviations from the
combustion plant, the combustion process itself and the loads methodological prescriptions of EN 15804 cannot be
and benefits of the substitution of fossil fuels and/or electricity. excluded but are considered not significant in the
Substitution effects in module D are always calculated for the context of this EPD.
net amount of secondary material or secondary fuel of the
3.7 Period under review
product system in line with EN 16485.
The company data gathered for this EPD represents the year
3.3 Estimates and assumptions 2020/21.
For the quantification of the net flows of recycled wood (input of
3.8 Geographic Representativeness
post­consumer wood used as a fuel minus post­consumer
wood exiting the product system into module D for energy Land or region, in which the declared product system is
recovery), it was assumed that all inputs of post­consumer manufactured, used or handled at the end of the product´s
wood are used as a fuel; inputs of post­consumer wood beyond lifespan: Europe
the need of wood fuel used in production was considered to be
used as a recycled material input.
3.9 Allocation
Beyond that, no relevant estimates or assumptions had to be
The inventories for the wood inputs were taken from ecoinvent
made beyond the information provided in this EPD.
v3.8. In ecoinvent, the forestry processes are modelled on a
3.4 Cut-off criteria mass­basis and sawmilling processes are allocated based on
revenues of the different co­products of a joint co­production
All data were taken into account that resulted from the data
process.
collection procedure in the plants, e.g. related to fuels, raw
Waste generated by edge­trimming and cut­size saws is used
material input, use of ancillary materials, waste flows,
internally for energy generation. Some plants sell minor
emissions into the air, water use, waste water, transport means
quantities of bark or electricity from co­generation. No impacts
and transport distances, etc..
are allocated to these outputs.
Expenses for the general management, research &
Biogenic carbon (content) is modelled manually thus reflects
development, administration and marketing – if known – were
the real physical flows; this is not the case for primary energy,
not taken into account.
implying that the content of primary energy in products and
The production of eventual packaging of ancillary material or
packaging is allocated as the main inputs/outputs of a unit
other inputs used during production (and some of the reported
process.
wastes) were generally neglected; in most cases reusable bins
In the case of sites where several products were produced and
or containers are used. In addition, the amounts of reported
no product­specific information was available, all inputs and
(unspecific) wastes are so small that their production can be
outputs related to production processes were attributed based
considered not relevant for the life cycle assessment. Additional
on a total mass of production; packaging material was
plant specific information can be found in the respective
attributed based on a total volume of the production. Inputs and
chapters for each plant.
outputs for coating processes that could not be separated from
Beyond that some plants reported ancillary materials that were
the data on plant level were conservatively attributed to the
cut off due to very small amounts and as inputs not directly
5 Environmental Product Declaration ­ Sonae Arauco, S.A. ­ Medium density fibreboard (MDF), uncoated
production of MDF. disregarded.
Post­consumer secondary wood is used as an input to produce No co­product allocation was made in the modelling of the
particleboard; for this input as well as for the end­of­life foreground data of the life cycle assessment underlying this
scenario, the end­of­waste status was defined after the sorting EPD.
and chipping of the wood­based board in line with EN 16485
(see also clause 3.2). In analogy, MDF leaving the product 3.10 Comparability
system at the end­of­life is considered a secondary fuel; its Basically, a comparison or an evaluation of EPD data is only
combustion and the benefits of energy recovery are declared in possible if all the data sets to be compared were created
module D. according to EN 15804 and the building context, respectively
Waste packaging in module A5 was considered not to reach the the product­specific characteristics of performance, are taken
end­of­waste state as a fuel. Its incineration is reported in A5, into account.
the benefits of energy recovery in module D. The benefits of the ecoinvent v3.8 (cut­off by classification) has been used as the
recycling of minor amounts of packaging materials are background database.
4. LCA: Scenarios and additional technical information
electricity (according to specifications of MWI plants in
Characteristic product properties of biogenic carbon ecoinvent v3.8).
Note: 1 kg of biogenic carbon is equivalent to 44/12 kg of CO .
2
Deconstruction (C1)
Information on describing the biogenic carbon content at
Manual deconstruction is assumed. The declared values are
factory gate
thus 0.
Name Value Unit
Biogenic carbon content in product 311 kg C Transport to waste treatment (C2)
Biogenic carbon in packaging 24,7 kg C This module includes the transport of the de­constructed
product to a recycling centre by a lorry (15 % emissions class
EURO 5; 85 % emissions class EURO 6) by over 50 km.
The following technical information is a basis for the declared
modules or can be used for developing specific scenarios in the
Waste treatment (C3)
context of a building assessment if modules are not declared
917 kg of uncoated MDF are chipped and exported from the
(MND).
product life cycle into module D, assuming a moisture content
of 20 % and a lower heating value of 18.0 MJ/kg. The biogenic
Transport to the construction site (A4)
carbon stored in the product and the content of primary energy
The product is transported from the production site to the
are exported from the product system as material inherent
construction site by a lorry (15 % emissions class EURO 5; 85
properties.
% emissions class EURO 6) over a default distance of 460 km.
Disposal (C4)
Installation into the building (A5)
This module is not relevant for the assumed end­of­life
Eventual further inputs for the installation of the products are
scenario. The declared values are thus 0.
not considered due to the broad applicability of the assessed
products.
Reuse, recycling, recovery potential (D)
An average transport distance of 30 km was assumed for
According to default assumptions in other IBU EPDs, post­
packaging waste from the construction site to the recycling
consumer wood is used as a secondary fuel for energy
plant or to the municipal waste incineration plant. The municipal
recovery in a biomass combustion plant with an overall energy
waste incineration plant is assumed to have an overall energy
efficiency of 93 % related to the lower heating value of the fuel
efficiency of 53 % related to the lower heating value of the
input; 91 % of the recovered energy is heat, 9 % is electricity.
waste input; 92 % of the recovered energy is heat, 8 % is
6 Environmental Product Declaration ­ Sonae Arauco, S.A. ­ Medium density fibreboard (MDF), uncoated
5. LCA: Results
DESCRIPTION OF THE SYSTEM BOUNDARY (X = INCLUDED IN LCA; MND = MODULE OR INDICATOR NOT DECLARED; MNR
= MODULE NOT RELEVANT)
Benefits and
Construction loads beyond
Product stage Use stage End of life stage
process stage the system
boundaries
la ire ta m w a Ry lp p u s tro p s n a rT g n iru tc a fu n a M e h t m o rf tro p s n a rTe tis e h t o t e ta g y lb m e s s A e s U e c n a n e tn ia M ria p e R tn e m e c a lp e R tn e m h s ib ru fe R y g re n e la n o ita re p Oe s u re ta w la n o ita re p Oe s u n o itc u rts n o c ­e Dn o itilo m e d tro p s n a rT g n is s e c o rp e ts a W la s o p s iD ­e s u e R­y re v o c e R­g n ilc y c e Rla itn e to p
A1 A2 A3 A4 A5 B1 B2 B3 B4 B5 B6 B7 C1 C2 C3 C4 D
X X X X X MND MND MNR MNR MNR MND MND X X X X X
RESULTS OF THE LCA - ENVIRONMENTAL IMPACT according to EN 15804+A2: Medium density fibreboard (MDF), uncoated,
per m³
Parameter Unit A1-A3 A4 A5 C1 C2 C3 C4 D
GWP­total kg CO 2 eq ­5.75E+02 5.84E+01 2.67E+01 0 8.3E+00 1.15E+03 0 ­5.93E+02
GWP­fossil kg CO 2 eq 5.87E+02 5.84E+01 2.02E+00 0 8.29E+00 7.45E+00 0 ­5.93E+02
GWP­biogenic kg CO 2 eq ­1.16E+03 0 2.47E+01 0 0 1.14E+03 0 0
GWP­luluc kg CO 2 eq 1.62E+00 2.33E­02 1.76E­04 0 3.92E­03 1.71E­02 0 ­2.96E­01
ODP kg CFC11 eq 6.91E­05 1.35E­05 1.83E­07 0 1.87E­06 3.74E­07 0 ­1.09E­04
AP mol H+ eq 3.95E+00 1.77E­01 9.24E­03 0 2.49E­02 3.98E­02 0 ­8.59E­01
EP­freshwater kg P eq 2.45E­02 4.15E­04 5.7E­06 0 6.77E­05 7.72E­04 0 ­1.31E­02
EP­marine kg N eq 7.25E­01 3.87E­02 4.11E­03 0 5.22E­03 5.4E­03 0 ­9.52E­02
EP­terrestrial mol N eq 9.56E+00 4.3E­01 4.62E­02 0 5.82E­02 6.17E­02 0 ­1.05E+00
kg NMVOC
POCP 3.93E+00 1.56E­01 1.38E­02 0 2.11E­02 1.74E­02 0 ­4.49E­01
eq
ADPE kg Sb eq 6.04E­03 2.06E­04 1.62E­06 0 3.8E­05 2.05E­05 0 ­3.27E­04
ADPF MJ 1.02E+04 8.85E+02 1.08E+01 0 1.24E+02 1.55E+02 0 ­1.42E+04
m3 world eq
WDP 6.54E+02 2.69E+00 9.11E­02 0 4.12E­01 1.8E+00 0 ­1.88E+01
deprived
GWP = Global warming potential; ODP = Depletion potential of the stratospheric ozone layer; AP = Acidification potential of land and water; EP =
Eutrophication potential; POCP = Formation potential of tropospheric ozone photochemical oxidants; ADPE = Abiotic depletion potential for non­fossil
resources; ADPF = Abiotic depletion potential for fossil resources; WDP = Water (user) deprivation potential)
RESULTS OF THE LCA - INDICATORS TO DESCRIBE RESOURCE USE according to EN 15804+A2: Medium density fibreboard
(MDF), uncoated, per m³
Parameter Unit A1-A3 A4 A5 C1 C2 C3 C4 D
PERE MJ 3.3E+03 1.24E+01 3.25E+02 0 2.06E+00 2.7E+01 0 ­4.67E+02
PERM MJ 1.21E+04 0 ­3.24E+02 0 0 ­1.18E+04 0 0
PERT MJ 1.54E+04 1.24E+01 1.69E­01 0 2.06E+00 ­1.18E+04 0 ­4.67E+02
PENRE MJ 8.14E+03 8.86E+02 2.83E+01 0 1.24E+02 1.57E+02 0 ­1.41E+04
PENRM MJ 2.03E+03 0 ­1.76E+01 0 0 ­2.01E+03 0 0
PENRT MJ 1.02E+04 8.86E+02 1.08E+01 0 1.24E+02 ­1.85E+03 0 ­1.41E+04
SM kg 0 0 0 0 0 0 0 0
RSF MJ 1.07E+03 0 0 0 0 0 0 1.05E+04
NRSF MJ 0 0 0 0 0 0 0 2.01E+03
FW m3 1.58E+01 9.37E­02 9.23E­03 0 9.23E­03 9.48E­02 0 ­1.17E+00
PERE = Use of renewable primary energy excluding renewable primary energy resources used as raw materials; PERM = Use of renewable primary
energy resources used as raw materials; PERT = Total use of renewable primary energy resources; PENRE = Use of non­renewable primary energy
excluding non­renewable primary energy resources used as raw materials; PENRM = Use of non­renewable primary energy resources used as raw
materials; PENRT = Total use of non­renewable primary energy resources; SM = Use of secondary material; RSF = Use of renewable secondary fuels;
NRSF = Use of non­renewable secondary fuels; FW = Use of net fresh water
RESULTS OF THE LCA – WASTE CATEGORIES AND OUTPUT FLOWS according to EN 15804+A2:
Medium density fibreboard (MDF), uncoated, per m³
Parameter Unit A1-A3 A4 A5 C1 C2 C3 C4 D
HWD kg 1.35E­02 2.31E­03 8.74E­06 0 3.33E­04 7.22E­05 0 ­1.54E­02
NHWD kg 1.19E+02 4.65E+01 2.59E­01 0 5.32E+00 1.03E+00 0 1.06E+01
RWD kg 4.81E­02 1.28E­02 1.43E­04 0 1.78E­03 2.04E­03 0 ­4.51E­02
CRU kg 0 0 0 0 0 0 0 0
MFR kg 3.02E+00 0 1.09E+00 0 0 0 0 0
MER kg 0 0 0 0 0 8.42E+02 0 0
EEE MJ 6.01E­01 0 1.11E+01 0 0 0 0 0
EET MJ 6.92E+00 0 1.28E+02 0 0 0 0 0
7 Environmental Product Declaration ­ Sonae Arauco, S.A. ­ Medium density fibreboard (MDF), uncoated
HWD = Hazardous waste disposed; NHWD = Non­hazardous waste disposed; RWD = Radioactive waste disposed; CRU = Components for re­use;
MFR = Materials for recycling; MER = Materials for energy recovery; EEE = Exported electrical energy; EET = Exported thermal energy
RESULTS OF THE LCA – additional impact categories according to EN 15804+A2-optional:
Medium density fibreboard (MDF), uncoated, per m³
Parameter Unit A1-A3 A4 A5 C1 C2 C3 C4 D
Disease
PM 3.15E­05 3.74E­06 1.3E­07 0 4.57E­07 1.21E­07 0 ­1E­06
incidence
IR kBq U235 eq 2.24E+01 3.84E+00 4.31E­02 0 5.4E­01 1.37E+00 0 ­2.58E+01
ETP­fw CTUe 1.61E+04 6.94E+02 1.77E+01 0 1.01E+02 8.81E+01 0 ­1.21E+03
HTP­c CTUh 4.29E­06 2.24E­08 4.83E­09 0 3.67E­09 4.18E­09 0 1.25E­07
HTP­nc CTUh 9.25E­06 7.06E­07 2.03E­08 0 9.88E­08 7.57E­08 0 ­2.23E­07
SQP SQP 8.48E+04 6.16E+02 2.18E+00 0 7.34E+01 2.39E+01 0 ­4.38E+02
PM = Potential incidence of disease due to PM emissions; IR = Potential Human exposure efficiency relative to U235; ETP­fw = Potential comparative
Toxic Unit for ecosystems; HTP­c = Potential comparative Toxic Unit for humans (cancerogenic); HTP­nc = Potential comparative Toxic Unit for humans
(not cancerogenic); SQP = Potential soil quality index
Disclaimer 1 – for the indicator “Potential Human exposure efficiency relative to U235”. This impact category deals mainly with the
eventual impact of low­dose ionizing radiation on human health of the nuclear fuel cycle. It does not consider effects due to possible
nuclear accidents, occupational exposure or radioactive waste disposal in underground facilities. Potential ionizing radiation from the
soil, radon and from some construction materials is also not measured by this indicator.
Disclaimer 2 – for the indicators “abiotic depletion potential for non­fossil resources”, “abiotic depletion potential for fossil resources”,
“water (user) deprivation potential, deprivation­weighted water consumption”, “potential comparative toxic unit for ecosystems”,
“potential comparative toxic unit for humans – cancerogenic”, “Potential comparative toxic unit for humans ­ not cancerogenic”,
“potential soil quality index”. The results of this environmental impact indicator shall be used with care as the uncertainties on these
results are high as there is limited experience with the indicator.
6. LCA: Interpretation
Figure 1 illustrates the contribution of each life cycle stage to fibre board (MDF).
the overall indicator results of the impact assessment (impact
from module A1 – C4 = 100 %) for uncoated medium density
Minor contributions stem from transport to the construction site
Figure 1: Environmental impacts of uncoated medium whereas the contributions from other modules of the life cycle
density fibreboard (MDF) along its life cycle (impacts from are negligible.
production modules A1 – C4 = 100 %) Loads and benefits beyond the life cycle (module D) are
negative (benefits > loads) whereas major contributions occur
Figure 1 illustrates that the environmental profile of uncoated for the ODP, the GWP­fossil and for the ADPF; these benefits
MDF is dominated by the production phase (modules A1 – A3). basically stem from the use of the MDF as secondary fuel and
8 Environmental Product Declaration ­ Sonae Arauco, S.A. ­ Medium density fibreboard (MDF), uncoated
its related substitution of natural gas and electricity from the
grid from the recovered energy.
Figure 2 illustrates that the biogenic carbon stored in the
uncoated MDF, expressed as CO ­equivalent, is higher than
2
the CO emissions from fossil sources, leading to a negative
2
GWP for the production module A1 – A3. The potential
substitution effect in mod­ule D almost offsets the GHG
emissions during the production phase (module A1­A3).
Figure 2: Greenhouse Gas balance of uncoated medium
density fibreboard (MDF)
The GWP is dominated by CO emissions and removals. [...]
2
7. Requisite evidence
Result: VOC emissions were tested for MDF according to
7.1 Formaldehyde several regulations.
A classification of A was achieved for French VOC regulation
For UF/MUF bonded boards: (Regulation of March and May 2011 DEVL1101903D and
DEVL1104875A)
Measuring agency: Aidimme Technology Institute, Valencia, AgBB/ABG requirements were complied (Anforderungen an
Spain bauliche Anlagen bezüglich de Gesundheitsschutzes (AGB).
Test report, date: no. 221.I.2303.329.EN.01 issued on the Entwurt 31.08.2017/August 2018 (AgBB))
15.03.2023
Overview of Results (28 days)
Result: Formaldehyde emission testing according to ASTM
Name Value Unit
D6007-14 was performed using EN 717 for formaldehyde
concentration determination. A value of 0,074 ppm was TVOC (C6 ­ C16) 27 μg/m3
determined. Sum SVOC (C16 ­ C22) < 5 μg/m3
R (dimensionless) 0.59 ­
Measuring agency: MPA Eberswalde, Materialprüfanstalt
VOC without NIK < 5 μg/m3
Brandenburg GmbH, Germany
Test report, date: No. 31/23/4267/01/QT issued on the Carcinogenic Substances < 1 μg/m3
17.04.2023
Result: Determination of formaldehyde release of wood­based AgBB overview of results (3 days [µg/m³])
panels according to: Name Value Unit
CARB final regulation order of "Airborne toxic control measure TVOC (C6 ­ C16) 230 μg/m3
to reduce formaldehyde emission from composite Wood
Sum SVOC (C16 ­ C22) < 5 μg/m3
products" and EPA TSCA Title VI 40 CFR Part 770.
Formaldehyde analysis by photometry by acetyl/acetone R (dimensionless) 0.88 ­
method according to EN 717-1. VOC without NIK 0.033 μg/m3
The requirement of CARB and EPA TSCA VI was met. Carcinogenic Substances < 1 μg/m3
7.2 Checking for the pre-treatment of the substances used
7.4 PCP/Lindane
No post­consumer wood is used in the production of Sonae Measuring agency: MPA Eberswalde, Materialprüfanstalt
Arauco MDF . Brandenburg GmbH, Germany
Test report, date: 31/21/2228/01PL issued at 15.04.2021
7.3 VOC emissions Result: Neither PCP nor Lindan content were detected. This
Measuring agency: Eurofins Denmark means that neither PCP nor Lindan were present in a quantity
Test report, date: 392­2019­00286101_A_EN issued in above the the method limit of quantification.
30.09.2019
9 Environmental Product Declaration ­ Sonae Arauco, S.A. ­ Medium density fibreboard (MDF), uncoated
8. References
Product category rules of IBU
EN 13501
IBU (2021) EN 13501­1:2019, Fire classification of construction products
IBU (2021): General Instructions for the EPD Programme of the and building elements – Classification using test data from
Institut Bauen und Umwelt e.V. (General Instructions for the reaction to fire tests.
IBU EPD Programme). Version 2.0, Institut Bauen und Umwelt,
Berlin. EN 13986
EN 13986:2015, Wood­based panels for use in construction –
IBU (2021) Characteristics, evaluation of conformity and marking.
IBU (2021): PCR Part A: Calculation rules for the life cycle
assessment and requirements for the project report according EN 14964
to EN 15804+A2:2019. Version 1.3, Institut Bauen und Umwelt, EN 14964:2006, Rigid underlays for discontinuous roofing –
Berlin. Definitions and characteristics.
IBU (2023) EN 15804
IBU (2023): PCR Part B: Requirements on the EPD for wood­ EN 15804+A2:2019 + AC:2021, Sustainability of construction
based panels. Version 2023/04, Institut Bauen und Umwelt, works ­ Environmental product declarations ­ Core rules for the
Berlin. product category construction products.
Standards and legal documents EN 16485
EN 16485:14­07, Round and sawn timber – Environmental
ASTM D6007 Product Declarations – Product category rules for wood and
ASTM D6007­14, Standard Test Method for Determining wood­based products for use in construction.
Formaldehyde Concentrations in Air from Wood Products Using
a Small­Scale Chamber. ISO 9001
ISO 9001:2015, Quality management systems – Requirements.
EN 310
EN 310:1993, Wood­based panels – Determination of modulus ISO 14001
of elasticity in bending and of bending strength. ISO 14001:2015, Environmental management systems –
Requirements with guidance for use.
EN 316
EN 316:2009, Wood fibre boards – Definition, classification and ISO 14025
symbol. ISO 14025:2006­07, Environmental labels and declarations –
Type III Environmental declarations – Principles and
EN 319 procedures.
EN 319:1993, Particleboards and fibreboards – Determination
of tensile strength perpendicular to the plane of the board. ISO 14044
EN ISO 14044:2006­07, Environmental management – Life
EN 322 cycle assessment – Requirements and guidance (ISO
EN 322:1993, Wood­based panels – Determination of moisture 14044:2006); German and English versions EN ISO
content. 14044:2006.
EN 323 ISO 16000
EN 323:1993, Wood­based panels – Determination of density. ISO 16000­11:2006, Indoor air – Part 11: Determination of the
emission of volatile organic compounds from building products
EN 324 and furnishing – Sampling, storage of samples and preparation
EN 324­1:1993, Wood­based panels – Determination of of test specimens.
dimensions of boards – Determination of thickness, width and
length. ISO 16895
EN 324­2:1993, Wood­based panels – Determination of ISO 16895­1:2008, Wood­based panels – Dry­process
dimensions of boards – Determination of squareness and edge fibreboard – Part 1: Classifications.
straightness. ISO 16895­2:2010, Wood­based panels – Dry­process
fibreboard – Part 2: Requirements.
EN 622
EN 622­1:2003, Fibreboards – Specifications – Part 1: General ISO 45001
requirements. ISO 45001:2018­06, Occupational health and safety
EN 622­5:2009, Fibreboards – Specifications – Part 5: management systems – Requirements with guidance for use.
Requirements for dry process boards (MDF).
ISO 50001
EN 717-1 ISO 50001:2018, Energy management systems –
EN 717­1:2005­01, Wood­based panels – Determination of Requirements with guidance for use.
formaldehyde release – Formaldehyde emission by the
chamber method. ChemVerbotsV
Verordnung über Verbote und Beschränkungen des
EN 12524 Inverkehrbringens und über die Abgabe bestimmter Stoffe,
EN 12524:2000, Building materials and products – Gemische und Erzeugnisse nach dem Chemikaliengesetz
Hygrothermal properties – Tabulated design values. (Chemikalien­Verbotsverordnung ­ ChemVerbotsV);
10 Environmental Product Declaration ­ Sonae Arauco, S.A. ­ Medium density fibreboard (MDF), uncoated
Ausfertigungsdatum: 20.01.2017. products and repealing Council Directive 89/106/EEC.
COUNCIL REGULATION (EU) No 333/2011 Regulation on the European Waste List (Waste index)
COUNCIL REGULATION (EU) No 333/2011 of 31 March 2011 http://www.gesetze­im­internet.de/avv/anlage.html
establishing criteria determining when certain types of scrap
metal cease to be waste under Directive 2008/98/EC of the Additional references
European Parliament and of the Council.
BBSR 2017
ECHA candidate list Bundesinstitut für Bau­, Stadt­ und Raumforschung Service Life
The Candidate List of substances of very high concern of Building Components; version 24.02.2017.
published by the European Chemicals Agency (ECHA), https://www.nachhaltigesbauen.de/fileadmin/pdf/Nutzungsdauer
Helsinki, available via https://echa.europa.eu/nl/­/four­ _Bauteile/BNB_Nutzungsdauern_von_Bauteilen_2017­02­
newsubstances­added­to­the­candidate­list 24.pdf
Regulation on biocidal products ecoinvent v3.8
REGULATION (EU) No 528/2012 OF THE EUROPEAN LCA database ecoinvent v3.8, Ökobilanzdatenbank, 12/2021.
PARLIAMENT AND OF THE COUNCIL of 22 May 2012 ecoinvent centre, Zürich.
concerning the making available on the market and use of
biocidal products. Weidema et al. (2013)
Weidema, B., C. Bauer, R. Hischier, C. Mutel, T. Nemecek, J.
Regulation (EU) Nr. 305/2011(CPR) Reinhard, C.O. Vadenbo, G. Wernet (2013): Overview and
REGULATION (EU) No 305/2011 OF THE EUROPEAN methodology, Data quality guideline for the ecoinvent database
PARLIAMENT AND OF THE COUNCIL of 9 March 2011 laying version 3. ecoinvent report no. 1 (v3), St. Gallen (CH).
down harmonised conditions for the marketing of construction
11 Environmental Product Declaration ­ Sonae Arauco, S.A. ­ Medium density fibreboard (MDF), uncoated
Publisher
Institut Bauen und Umwelt e.V. +49 (0)30 3087748­ 0
Hegelplatz 1 info@ibu­epd.com
10117 Berlin www.ibu­epd.com
Germany
Programme holder
Institut Bauen und Umwelt e.V. +49 (0)30 3087748­ 0
Hegelplatz 1 info@ibu­epd.com
10117 Berlin www.ibu­epd.com
Germany
Author of the Life Cycle Assessment
Dr. Frank Werner ­ Umwelt & Entwicklung + 41 (0)44 241 39 06
Kammelenbergstrasse 30 frank@frankwerner.ch
9011 St. Gallen http://www.frankwerner.ch/
Switzerland
Owner of the Declaration
Sonae Arauco, S.A. (+34) 918 070 701
Calle Ulises 26­18 products@sonaearauco.com
28043 Madrid www.sonaearauco.com
Spain
12 Environmental Product Declaration ­ Sonae Arauco, S.A. ­ Medium density fibreboard (MDF), uncoated
