Environmental Product
Declaration
as per ISO 14025 and EN 15804
Owner of the declaration: MINIERA SAN ROMEDIO SRL
Publisher: Kiwa-Ecobility Experts
Programme operator: Kiwa-Ecobility Experts
Registration number: EPD-Kiwa-EE-330-EN
Issue date: 24.10.2023
Valid to: 24.10.2028
Heavy cement mortar: PAVI RAPID,
PAVI RAPID LOW, PAVI PRONTO, T
BLOCK, T SPAN, T CREAM, PAVI
TEKNO, DRAINMASS, BETONTASS
DE
Ready-to-use mortars based on dolomia
and Portland cement.
1. General information
Miniera San Romedio Heavy cement mortar
Programme operator Owner of the declaration
Kiwa-Ecobility Experts Miniera San Romedio Srl
Kiwa GmbH, Ecobility Experts Località alla Miniera
Wattstraße 11-13 38012 Predaia (TN)
13355 Berlin Italy
Germany
Registration number Declared product / declared unit
EPD-Kiwa-EE-330-EN 1 ton (1000 kg) of heavy cement mortar
This declaration is based on the Product Scope
Category Rules This EPD refers to a single product (Heavy ce-
EN 16908:2017+A1:2022 ment mortar) produced by Miniera San Rome-
dio Srl in its plants in the province of Trento
Issue date (Italy). The data used to perform the LCA anal-
24.10.2023 ysis were provided by Miniera San Romedio Srl
and referred to the production of one year,
Valid to and the information are relative to the period
24.10.2028 2021-2022. The geographical area assumed
for the application and end-of-life of the prod-
uct is Italy. The study was performed following
the so-called from-cradle-to-gate approach
with modules C1-C4 and D.
This EPD is intended to be used for business-
to-consumer communications. The owner of
the declaration is liable for the underlying in-
formation and evidence.
Kiwa-Ecobility Experts assumes no liability for
manufacturer's information, LCA data and ev-
idence.
Verification
The European standards EN 15804+A2:2019
(10/2021) serve as PCR.
Independent verification of the declaration
and data according to ISO 14025:2006.
☐internal ☒external
Frank Huppertz
(Head of Kiwa-Ecobility Experts)
Prof. Dr. Frank Heimbecher Dr.-Ing. Morteza Nikravan
(Chairman of the independent expert committee – (External verifier of Kiwa GmbH)
Kiwa-Ecobility Experts)
Page | 2 Miniera San Romedio — Heavy cement mortar
2. Product
2.1 Product description
The premixed Miniera San Romedio’s products are inorganic finely grinded materials, obtained by
means of the combinations at different relative concentrations of natural hydraulic lime, cement and
dolomia. In this EPD the Heavy cement mortar is considered.
2.2 Application
Heavy cement mortar: a ready-to-use mortar based on dolomia and Portland cement produced ac-
cording to EN1504-3.
2.3 Technical data
In Table 1 the main physical and applicative properties of the considered product are reported.
Table 1: Physical and applicative properties of the Heavy cement mortar.
Characteristic Unit Value Standard
Density kg/m3 1650-2080 UNI EN 1015-10
Mixing water l/kg 0.07-0.21 -
Max granulometry mm 1-4 EN 1015-1
2.4 Placing on the market/ Application rules
The pre-mixed Miniera San Romedio’s products are powder or granulates and therefore they have to
be transported to the building site by using 25 kg paper bags, collected over a pallet. Pallets range from
50 to 60 bags each one, and can be mechanically moved. Once the product reaches the building site
the bags can be used to mix the product with the specified amount of water and either be manually
stirred or mechanically mixed. It can be also transported to the construction site unpackaged and di-
rectly pumped into a silo already settled on a nearby position.
2.5 Base materials / Ancillary materials
In order to apply this product, it must be premixed combining at different relative concentrations ce-
ment and fillers (i.e dolomia). Water and small amounts of additives (less than 3 wt%) are then added
to the mix, in order to develop inno-vative materials with very peculiar properties and suitable for a
wide range of applications in the con-structions field. The relative composition of the Heavy cement
mortar is summarized in Table 2.
Table 2: Composition of Heavy cement mortar.
Product Dolomia NHL* Cement Hydrated lime Additives
[wt%] [wt%] [wt%] [wt%] [wt%]
Heavy cement mortar 80-90 - 10-20 - < 3
* Comprising setting retardant (4 wt% of the total NHL content)
The paper bag used as packaging (2.74 kg for 1 ton of product) contains 1.77 kg of biogenic carbon.
The product does not contain biogenic carbon.
2.6 Manufacturing
2.6.1 Manufacturing process of the inert
The Dolomia is extracted in the Rio Maggiore pit through a mixed explosive. The material is then col-
lected through a Diesel bulldozer and transported to Mollaro (TN) with a Diesel lorry where the mate-
rial is subjected to a first crushing. The material is then dried and crushed for a second time using an
hammer mill.
Page | 3 Miniera San Romedio — Heavy cement mortar
2.6.2 Manufacturing of the premixed products
The powders (cement, hydrated lime and dolomia) are then mixed and packed through a bagging sys-
tem, by using a paper bag with capacity of 25 kg, palletized and then directly distributed.
According to the EN 15804:2012+A2:2019 standard, the present LCA study was performed following
the so-called from-cradle-to-gate approach with modules C1-C4 and D considering thus the following
steps:
● Extraction and processing of the raw materials (A1);
● Transport of the acquired raw materials to the manufacturer and internal transport of the ex-
tracted raw materials (A2);
● Production of the materials and mixing operations (A3).
● Deconstruction/demolition (C1)
● Transport of demolition wastes (C2)
● Waste treatment (C3)
● Waste disposal (C4)
● Benefits and impacts beyond the system boundaries (D)
A schematic process flow diagram is shown in Figure 1.
Figure 1: [Graphic schematic process flow diagram for the analysed product.]
* hydrated lime is not present in all compositions, please refer to Table 2.
2.7 Packaging
Paper bags are used to stow 25 kg of premixed product.
2.8 Reference Service Life (RSL)
Since the use phase is not considered, the reference service life (RSL) as per ISO 15686-1, -2, -7 and -8
has not been declared.
2.9 Other Information
For further information on this product please visit the webpage under the following link:
https://www.tassullo.it/it/
Page | 4 Miniera San Romedio — Heavy cement mortar
3. LCA: Calculation rules
3.1 Declared unit
In accordance with the EN 15804+A2:2019 and EN 16908:2017+A1 1 ton of product is chosen as the
declared unit (see Table 3).
Table 3: Declared unit used for the calculations.
Product Unit Value
Declared Unit ton 1
Conversion factor to 1 kg kg 1000
3.2 System boundary
In accordance with the EN 15804+A2:2019 this study was performed following the so-called from-cra-
dle-to-gate approach with modules C1-C4 and D. In Table 4 the system boundaries of the considered
product are listed.
Table 4: system boundaries of the heavy cement mortar.
Modul within the Outside the system
Module
declared system boundary boundary
A1 Raw Material Yes X
A2 Transport Yes X
A3 Manufacturing Yes X
A4 Transport No X
A5 Installation No X
B1 Use Phase No X
B2 Maintance No X
B3 Repair No X
C1 De-Construction Yes X
C2 Transport Yes X
C3 Waste treatment Yes X
C4 Landfill Yes X
D Considered loads and Yes X
benefits outside of the sys-
tem boundary in Module D
3.3 Estimates and assumptions
The electrical energy consumed in Miniera San Romedio Srl plants is a fully renewable certified energy.
The electrical energy is derived from renewable energy source (hydropower) that have obtained cer-
tification with the certification of the renewability. The electrical energy is converted from high voltage
to low voltage using an electrical transformer located close to the plants. The certification of the re-
newability of the energy covers to whole period analysed in this study (2021-2022). For the internal
transportations, gasoline with a calorific power of 45 MJ/kg was considered.
For as concerns the end-of-life stage, the demolition, transport, treatment, and disposal of wastes
were modelled using processes present in the Ecoinvent database and modified to the specific case.
In particular,
• for the C1 stage (demolition/deconstruction) the use of a diesel operating machine with a
productivity of 16.6 min/ton of demolished material and a diesel consumption of 0.9 lt/m3 was
Page | 5 Miniera San Romedio — Heavy cement mortar
considered. A water consumption of 0.018 m3/m3 was considered. Both references were taken
from Ivanica et al.
• for the C2 stage a distance of 15 km was assumed according to data provided by Italia del
Riciclo referred to the year 2021.
• for the C3 and C4 stages, despite the heavy cement mortar can be fully recycled and due to
the lack of specific information regarding the end-of-life of this product, it was assumed that,
after a sorting and crushing process, 78.1 wt% of inert wastes is recycled (reaching the end-of-
waste state) while the remaining part is landfilled (data provided by Italia del Riciclo referred
to the year 2021). For the sorting and crushing process an existing Ecoinvent process was
adapted to the specific case.
• for the stage D it was considered that the secondary materials were used as alternative to
gravel for the production of concrete and for road construction (the background process used
refers to the period 2013-2021). Benefits and impacts associated to these operations were
therefore evaluated.
According to EN 16908:2017+A1 the carbonation of cement and hydrated lime can be very relevant
after demolition with consistent carbon dioxide uptake. The evaluation of carbon dioxide uptake was
carried out according to the procedure described in EN 16757. In particular it was considered that:
• for the C1-C3 stages no carbonation occurs due to the limited time of exposure to air or to the
lack of information regarding the duration of air exposure.
• for the C4 stage it was considered a carbon dioxide uptake equal to 75 % of the maximum
theoretical carbon dioxide uptake for landfilled wastes. No uptake was considered for recycled
wastes.
• for the D stage it was considered a carbon dioxide uptake equal to 100 % of the maximum
theoretical carbon dioxide uptake.
The following values (evaluated according to stoichiometry) were used as maximum uptake values:
• Cement: 490 kg CO /ton;
2
• Hydrated lime: 594 kg CO /ton.
2
It should be highlighted that since Miniera San Romedio produces ready mixed products and has no
control and no information regarding their applications it was impossible, due to lack of data, to cal-
culate the contribution of carbonation in the use stage (module B).
Regarding the end-of-life of the packaging paper (100 % recyclable), it was not considered since beyond
the boundaries of the system.
3.4 Cut-off Criteria
As reported in the EN 15804:2012+A2:2019 standard, all inputs and outputs for which data are availa-
ble were taken into account in the calculation. Eventual data gaps have been filled with conservative
assumptions of average data or generic data available in the Ecoinvent v3.8 database of the SimaPro
software. All flows contributing to more than 1 % of the total mass, energy or environmental impact
of the system have been included in the life cycle assessment. Eventual neglected processes do not
contribute in total more than 5% to the impact categories considered. Moreover, the manufacture of
machinery, plants and other infrastructure required for production of the products under review was
not taken into consideration in the present analysis.
Page | 6 Miniera San Romedio — Heavy cement mortar
3.5 Period under review and Geographical reference area
The specific data were obtained directly by the commissioning company, and are related to the pro-
duction of one year. The data are referred to the period June 2021-June 2022. They were obtained by
means of specific measures related to the energy consumption and mass flows in the plant of Mollaro
(Trento), where Dolomia is extracted, mixed with cement and packed. Manufacturer-specific data are
referred to the period 2021-2022, while generic data are less than 10 years old. Moreover, process-
specific data are based on the average of an operating year.
3.6 Data quality
For this study, the data quality requirements defined in ISO 14044 regulation have been considered.
In order to ensure coherence, data with the same level of detail have been used, as well as under the
same methodological considerations. Data and methods used for this study have been described with
the purpose of being reproducible by a third independent party. Whenever possible, generic data used
for the study are representative of the location where the process belongs (for example, the produc-
tion of electrical energy). The data has been collected from the plant of Mollaro (in province of Trento).
Data were associated to a specific input selected from the database Ecoinvent v3.8 (2021). The inven-
tory analysis has been thus modelled by using the SimaPro software.
3.7 Allocation
In this work, allocations have been avoided as far as possible (e.g. by system expansion, splitting pro-
cesses into sub-processes). Where it was necessary, an economical allocation principle was utilized.
This choice was performed because the economic difference between product and co-products was
rather elevated. In this sense, the environmental impacts associated with the inputs have been distrib-
uted according to the way they affect the subsequent production process.
A peculiar feature of the cave in Mollaro is that the extraction of the dolomia is performed for two
interconnected purposes: obtaining the inerts to be mixed with the NHL in the premixed products of
Tassullo, and creating the spaces to store the apples produced in Trentino by Melinda Spa company
and creating spaces to store alimentary products or to host other industrial activities, which is planned
for the near future. Because of this reason, the extraction of the dolomia from the plant of Mollaro is
subjected to a specific mineralogical design which takes into account the development of large cham-
bers. The necessity to apply a different mineralogical excavation technique, very far from the optimized
mining technique traditionally used for the extraction of the inerts, involves a larger demand of energy
and explosive. In particular the excavation for the storage of apples, taken as reference because prev-
alent storage activity, compared to the traditional optimized mining technique, implies a surplus of the
mining costs of the 79% for Miniera San Romedio Srl company. Therefore, in this study only the 21%
of the environmental impact coming from the extraction of the dolomia has been attributed to Miniera
San Romedio Srl, following the economical allocation principle, while the remaining part was consid-
ered as an input of the LCA system of Melinda Spa. On the other hand, all the operations related to
the subsequent crushing and transportation of dolomia have been fully attributed to the present sys-
tem, as the extracted dolomia is fully utilized by Miniera San Romedio Srl as inert material for the
preparation of pre-mixed products.
3.8 Comparability
In order to assure the comparability of the obtained results, all datasets to be compared have been
created in accordance with EN 15804, and the product-specific performance characteristics have been
taken into account. In principle, a comparison or assessment of the environmental impacts of different
products is only possible if they have been prepared in accordance with EN 15804.
Page | 7 Miniera San Romedio — Heavy cement mortar
4. LCA: Scenarios and additional technical information
No scenario or additional technical information to be declared.
5. LCA: Results
Table 5 shows the results of the impact assessment indicators, resource use, waste and other output
streams for the declared unit (1 ton of heavy cement mortar). The results presented here refer to the
declared product. In Table 6 the results of the biogenic carbon content are reported.
Disclaimer on ADP-e, ADP-f, WDP, ETP-fw, HTP-c, HTP-nc, SQP: The results of these environmental
impact indicators must be used with caution, as the uncertainties in these results are high or as there
is limited experience with the indicator.
Disclaimer on IR: This impact category mainly addresses the potential effect of low dose ionizing radi-
ation on human health in the nuclear fuel cycle. It does not consider effects due to possible nuclear
accidents and occupational exposures, nor does it consider radioactive waste disposal in underground
facilities. Potential ionizing radiation from soil, radon, and some building materials is also not measured
by this indicator.
Page | 8 Miniera San Romedio — Heavy cement mortar
Description of the system boundary
Construction process Benefits and loads beyond
Product stage Use stage End of life stage
stage the system boundaries
la ir e t a m w a Ry lp p u s t r o p s n a r T u n a M-g n ir u t c a f t r o p s n a r Tu n a m m o r-
f
o t r e r u t c a fe s u fo e c a lp n o it c u r ts n o
C
n o it a lla ts n -is s e c o r p e s U n ia M-e c n a n e t r ia p e R tn e m e c a lp e
R
r u fe R-n e m h s ib la n o it a r e p Oe s u y g r e n e la n o it a r e p Oe s u r e t a w e D- n o it c u r ts n o cn o itilo m e d
/
t r o p s n a r T e ts a Wg n is s e c o r p la s o p s iD e s u e R-y r e v o c e R- g n ilc y c e R- a itn e t o pl
A1 A2 A3 A4 A5 B1 B2 B3 B4 B5 B6 B7 C1 C2 C3 C4 D
X X X MND MND MNR MNR MNR MND MND MND MND X X X X X
X=Module declared | MND=Module not declared
LCA results - Indicators describing environmental impacts based on the impact assessment (LCIA): 1 ton of heavy cement mortar (EN 15804+A2)
Parameter Unit A1-A3 C1 C2 C3 C4 D
Core environmental impact indicators (EN 15804+A2)
GWP-total kg CO2 eqv. 1.54E+02 7.62E+00 1.37E+00 1.73E+00 -1.09E+01 -6.02E+01
GWP-f kg CO2 eqv. 1.53E+02 7.61E+00 1.37E+00 1.68E+00 -1.09E+01 -6.01E+01
GWP-b kg CO2 eqv. 9.42E-01 5.33E-03 1.39E-03 4.62E-02 1.25E-03 -1.11E-01
GWP-luluc kg CO2 eqv. 5.38E-02 1.13E-03 4.90E-04 3.51E-03 1.09E-03 -2.15E-03
ODP kg CFC 11 eqv. 7.07E-06 3.16E-06 3.31E-07 1.16E-07 4.67E-07 -3.55E-07
AP mol H+ eqv. 4.40E-01 3.65E-02 9.54E-03 1.04E-02 1.08E-02 -2.35E-02
EP-fw kg P eqv. 2.69E-02 3.03E-04 8.50E-05 1.50E-03 1.06E-04 -6.12E-04
EP-m kg N eqv. 1.14E-01 9.56E-03 3.74E-03 2.26E-03 3.77E-03 -6.73E-03
EP-T mol N eqv. 1.27E+00 1.05E-01 4.10E-02 2.18E-02 4.13E-02 -9.02E-02
POCP kg NMVOC eqv. 3.27E-01 3.41E-02 1.15E-02 6.05E-03 1.20E-02 -2.11E-02
ADP-mm kg Sb-eqv. 3.37E-04 4.85E-06 3.13E-06 1.47E-05 2.63E-06 -5.65E-05
ADP-f MJ 9.16E+02 1.99E+02 2.16E+01 3.39E+01 3.22E+01 -4.07E+01
WDP m3 world eqv. 3.12E+01 4.16E+00 7.31E-02 3.75E-01 1.45E+00 -8.13E-01
Additional environmental impact indicators (EN 15804+A2)
CaPM disease incidence ND ND ND ND ND ND
IR kBq U235 eqv. ND ND ND ND ND ND
ETP-fw CTUe ND ND ND ND ND ND
HTP-c CTUh ND ND ND ND ND ND
HTP-nc CTUh ND ND ND ND ND ND
SQP Pt ND ND ND ND ND ND
ADP-mm= Abiotic depletion potential for non-fossil resources | ADP-f=Abiotic depletion for fossil resources potential | AP= Acidification potential, Accumulated Exceedance | EP-fw = Eutrophication potential, fraction of nutrients reaching
freshwater end compartment | EP-m= Eutrophication potential, fraction of nutrients reaching marine end compartment| EP-T= Eutrophication potential, Accumulated Exceedance | GWP-b=Global Warming Potential biogenic | GWP-f=Global
Warming Potential fossil fuels | GWP-luluc=Global Warming Potential land use and land use change |GWP-total=Global Warming Potential total| ODP=Depletion potential of the stratospheric ozone layer |POCP=Formation potential of
tropospheric ozone | WDP=Water (user) deprivation potential, deprivation- weighted water consumption | ETP-fw=Potential Comparative Toxic Unit for ecosystems | HTP-c=Potential Toxic Unit for Humans toxicity, cancer | HTP-nc= Potential
Toxic Unit for humans, non-cancer | IRP=Potential Human exposure efficiency relative to U235, human health | PM=Potential incidence of disease due to Particulate Matter emissions | SQP=Potential soil quality index
Page | 9 Miniera San Romedio — Heavy cement mortar
Parameter Unit A1-A3 C1 C2 C3 C4 D
PERE MJ 2.36E+02 8.53E-01 2.71E-01 6.27E+00 2.75E-01 -1.30E+01
PERM MJ 0.00E+00 0.00E+00 0.00E+00 0.00E+00 0.00E+00 0.00E+00
PERT MJ 2.36E+02 8.53E-01 2.71E-01 6.27E+00 2.75E-01 -1.30E+01
PENRE MJ 9.70E+02 2.12E+02 2.29E+01 3.56E+01 3.42E+01 -4.27E+01
PENRM MJ 0.00E+00 0.00E+00 0.00E+00 0.00E+00 0.00E+00 0.00E+00
PENRT MJ 9.70E+02 2.12E+02 2.29E+01 3.56E+01 3.42E+01 -4.27E+01
SM Kg 0.00E+00 0.00E+00 0.00E+00 0.00E+00 0.00E+00 0.00E+00
RSF MJ 0.00E+00 0.00E+00 0.00E+00 0.00E+00 0.00E+00 0.00E+00
NRSF MJ 0.00E+00 0.00E+00 0.00E+00 0.00E+00 0.00E+00 0.00E+00
FW M3 3.01E+01 3.99E+00 7.35E-02 3.69E-01 1.45E+00 -7.11E-01
HWD Kg 1.33E-03 5.41E-04 5.23E-05 3.25E-05 4.87E-05 -1.76E-04
NHWD Kg 1.01E+01 1.79E-01 1.99E+00 1.22E-01 2.19E+02 -6.55E-01
RWD Kg 4.97E-03 1.40E-03 1.46E-04 2.45E-04 2.11E-04 -2.96E-04
CRU Kg 0.00E+00 0.00E+00 0.00E+00 0.00E+00 0.00E+00 0.00E+00
MFR Kg 1.80E-02 0.00E+00 0.00E+00 7.81E+02 0.00E+00 0.00E+00
MER Kg 0.00E+00 0.00E+00 0.00E+00 0.00E+00 0.00E+00 0.00E+00
EET MJ 0.00E+00 0.00E+00 0.00E+00 0.00E+00 0.00E+00 0.00E+00
EEE MJ 0.00E+00 0.00E+00 0.00E+00 0.00E+00 0.00E+00 0.00E+00
PERE=Use of renewable primary energy excluding renewable primary energy resources used as raw materials | PERM= Use of renewable primary energy resources used as raw materials | PERT=Total use of renewable primary energy
resources | PENRE= Use of non-renewable primary energy excluding non-renewable primary energy resources used as raw materials | PENRM= Use of non-renewable primary energy resources used as raw materials | PENRT= Total use
of non-renewable primary energy resources | SM=Use of secondary material | RSF=Use of renewable secondary fuels | NRSF=Use of non-renewable secondary fuels | FW=Use of fresh water | HWD=Hazardous waste disposed |
NHWD=Non-hazardous waste disposed | RWD=Radioactive waste disposed | CRU=Components for re-use | MFR=Materials for recycling | MER=Materials for energy recovery | EET=Exported energy, thermical | EE=Exported energy,
electrical
In Table 6 the biogenic content of heavy cement mortar is reported.
Table 6: results of the biogenic carbon content of heavy cement mortar.
LCA results - information on biogenic carbon content at the factory gate: 1 ton of heavy cement mortar (EN 15804+A2)
Parameter Unit Value
biogenic carbon content in product kg C 0
biogenic carbon content in accompanying packaging kg C 1.77
NOTE 1 kg biogenic carbon is equivalent to 44/12 kg CO2
Page | 10 Miniera San Romedio — Heavy cement mortar
6. References
ISO 14040:2006, Environmental management - Life cycle assessment - Principles and framework
ISO 14044:2006, Environmental management - Life cycle assessment - Requirements and guidelines
ISO 14025:2006: Environmental labels and declarations — Type III environmental declarations — Prin-
ciples and procedures EN 13249
EN 15804:2012+A2:2019 Sustainability of construction works — Environmental Product Declarations
— Core rules for the product category of construction products
PCR A: General Program Category Rules for Construction Products from the EPD program Kiwa-Ecobil-
ity Experts, R.0_2021-07-16
EN 16908:2017+A1: Cement and building lime - environmental product declarations - product category
rules complementary to EN 15804.
EN16757: Sustainability of construction works – Environmental product declarations – Product cate-
gory rules for concrete and concrete elements.
Ivanica, R., M. Risse, G. Weber-Blaschke, and K. Richter, Development of a life cycle inventory database
and life cycle impact assessment of the building demolition stage: A case study in Germany. Journal of
Cleaner Production, 2022. 338: p. 130631.
Frischknecht, R. and N. Jungbluth. Overview and Methodology. Ecoinvent report No. 1. 2007.
Fondazione per lo sviluppo sostenibile, F.U., Unione Imprese Economia Circolare,. L'Italia del Riciclo.
2021; Available from: https://www.cial.it/rapporto-italia-del-riciclo-2021/#:~:text=Se-
condo%20i%20dati%20Ispra%20sono,e%20il%2060%25%20al%202030.
Laveglia, A., L. Sambataro, N. Ukrainczyk, N. De Belie, and E. Koenders, Hydrated lime life-cycle assess-
ment: Current and future scenarios in four EU countries. Journal of Cleaner Production, 2022. 369
Page | 11 Miniera San Romedio — Heavy cement mortar
7. ANNEX 1 Requirements of the Minimum Environmental Criteria (DM June 23th 2022)
In Table 7 the requirements imposed by Minimum Environmental Criteria (DM June 23th 2022) for the
heavy cement mortar considered in this project report are summarized. As it can be seen, the product
satisfies the legislative requirements imposed by the Italian Legislation on the Minimum Environmen-
tal Criteria for construction services.
Table 7: Requirements of the Minimum Environmental Criteria DM June 23th 2022) for the heavy ce-
ment mortar.
2.5.1 Emissions in confined The required emission limits can
environment not be applied to these materi-
als since their applications are
not included in the list provided
in the DM June 23th 2022 at the
point 2.5.1.
2.5.2 Premixed concrete or The required minimum recycled
prepared on the building content is not applicable since
site the products considered in this
EPD can not be considered as
“concrete”. According to EN
998-1 and EN 998-2 they can be
defined as “plasters” or “mor-
tars” depending on the specific
application.
2.6.2 Dismantling and re- All the products considered in
moval of the materials this EPD, after the dismantling
operations, can be fully sent to
reuse, recovery and recycling
operations.
Note: the other requirements imposed by the Minimum Environmental Criteria are not reported since
not applicable for the analyzed products.
Page | 12 Miniera San Romedio — Heavy cement mortar
Publisher Mail DE.Ecobility.Ex-
Kiwa-Ecobility Experts perts@kiwa.com
Kiwa GmbH, Ecobility Experts Web https://www.kiwa.com/de/
Wattstraße 11-13 de/themes/ecobility-ex-
13355 Berlin perts/ecobility-experts/
Germany
Programme operator Mail DE.Ecobility.Ex-
Kiwa-Ecobility Experts perts@kiwa.com
Kiwa GmbH, Ecobility Experts Web https://www.kiwa.com/de/
Wattstraße 11-13 de/themes/ecobility-ex-
13355 Berlin perts/ecobility-experts/
Germany
LCA Practitioner Tel. (+39) 0461/283724
Prof. Andrea Dorigato, Ing. Fax. andrea.dorigato@unitn.it
Francesco Valentini Mail https://webapps.unitn.it/d
University of Trento Web u/it/Per-
Department of Industrial Engi- sona/PER0009668/Curricu-
neering (DII) lum
Via Sommarive 9
38123 Trento
Italy
Owner of the declaration Tel. (+39) 0463/662100
Miniera San Romedio Srl Fax. (+39) 0463/662113
Località alla Miniera Mail minierasanromedio@pec.it
38012 Predaia Web www.minierasanromedio.it
Italy VAT 00602230229
Kiwa-Ecobility Experts -
established member of
Page | 13 Miniera San Romedio — Heavy cement mortar
