ENVIRONMENTAL PRODUCT DECLARATION
as per ISO 14025 and EN 15804+A2
Owner of the Declaration MMFA - Multilayer Modular Flooring Association
Publisher Institut Bauen und Umwelt e.V. (IBU)
Programme holder Institut Bauen und Umwelt e.V. (IBU)
Declaration number EPD-MMF-20240106-CBG1-EN
Issue date 04.06.2024
Valid to 03.06.2029
Vinyl- HDF- floor covering
MMFA (Multilayer Modular Flooring
Association)
www.ibu-epd.com | https://epd-online.com
General Information
MMFA (Multilayer Modular Flooring Vinyl- HDF- floor covering
Association)
Programme holder Owner of the declaration
IBU – Institut Bauen und Umwelt e.V. MMFA - Multilayer Modular Flooring Association
Hegelplatz 1 Mittelstrasse 50
10117 Berlin 33602 Bielefeld
Germany Germany
Declaration number Declared product / declared unit
EPD-MMF-20240106-CBG1-EN 1 m² of Vinyl-HDF floor covering
This declaration is based on the product category rules: Scope:
Floor coverings, 01.08.2021 This Environmental Product Declaration (EPD) is an association EPD and
(PCR checked and approved by the SVR) refers to a representative Vinyl-HDF floor covering produced by European
manufacturers that are members of MMFA®.
Data are based upon production during 2022 in Europe. Data have been
Issue date provided by 4 companies of MMFA which represent 66% percent of MMFA
members.
04.06.2024
The declared Vinyl-HDF floor covering represents a weighted average of
best-selling products withing the thickness range of 9,1 - 10 mm, that
meets the requirements of the use classes: 21-23, 31-34 according to EN
Valid to
ISO 20326 or EN 16511, ISO 10874.
03.06.2029 The owner of the declaration shall be liable for the underlying information
and evidence; the IBU shall not be liable with respect to manufacturer
information, life cycle assessment data and evidences.
The EPD was created according to the specifications of EN 15804+A2. In
the following, the standard will be simplified as EN 15804.
Verification
The standard EN 15804 serves as the core PCR
Independent verification of the declaration and data according to ISO
14025:2011
Dipl.-Ing. Hans Peters
internally X externally
(Chairman of Institut Bauen und Umwelt e.V.)
Florian Pronold Mrs Kim Allbury,
(Managing Director Institut Bauen und Umwelt e.V.) (Independent verifier)
1 Environmental Product Declaration - MMFA (Multilayer Modular Flooring Association) - Vinyl- HDF- floor covering
Product
This product contains substances listed in the candidate list
Product description/Product definition (date: 25.08.2023) exceeding 0.1 percentage by mass: NO.
Vinyl-HDF floor coverings described in this EPD are produced
by member companies of MMFA®. The floor coverings meet Manufacturing
the requirements of EN ISO 20326 or EN 16511. The illustration below describes the manufacturing process of
Vinyl-HDF floorings consist of a number of layers. On the top the floor covering (simplified).
side there is a PVC-decor with a transparent, wear-resistant
contact surface which is varnished; in the middle there is a core
layer made of high-density wood fibres (HDF) and on the back
side there is a stabilizing layer to guarantee floor stability.
Certain product constructions offer as well integrated impact
sound insolation.
The decorative layer of a Vinyl-HDF floor covering can be
printed with any design and gives the floor its individual
appearance. For the placing on the market of the product in the
European Union/European Free Trade Association (EU/EFTA)
(with the exception of Switzerland) Regulation (EU) No.
305/2011 (CPR) applies. The product needs a declaration of
performance taking into consideration EN
Packaging
14041:2004+AC:2005+AC:2006 Resilient, textile and laminate
As packaging materials mainly wooden pallets, cardboard and
floor coverings – Essential characteristics and the CE-marking.
polyethylene-film are used. Wooden pallets can be used
For the application and use the respective national provisions
several times and can be recycled at the end of life.
apply.
Cardboards and polyethylene-films can be fed into the recycling
Application cycle in accordance with local regulations and possibilities and
thus be reused.
The Vinyl-HDF floor covering described in this EPD is intended
to be used within a building and meets the requirements of the
use classes: 21-23, 31-34 according to EN ISO 20326 or EN
Reference service life
16511, EN ISO 10874.
The estimated service life of a floor covering depends e.g. on
For the application and use the respective national provisions
the type of floor covering and the area of application, the user
apply.
and the maintenance of the product. Comparisons of different
Technical Data floor coverings are only allowed if these parameters are
considered in a consistent way. A minimum service life of 20
The following table contains the construction data of
years can be assumed, technical service life can be
the declared product group:
considerably longer (BNB refers to a service life of 20 years).
Constructional data The use stage is declared in this EPD for a one-year usage.
Name Value Unit
Product thickness 9.1 - 10 mm Extraordinary effect
Vinyl-HDF-floor coverings are normally in the reaction to fire
Grammage 850 - 980 g/m2
class Cfl-s1 according to EN 13501-1.
Product Form Panel -
Length of the surface layer 300 - 2500 mm Re-use phase
Width of the surface layer 70 - 600 mm Vinyl-HDF-panels are installed loose laid and do have a high
Length and width of squared elements 250 - 700 mm light resistance that delays a change in the decorative surface.
They can thus be re-used in another flooring installation in case
Density 930 - 970 kg/m3
of careful and selective dismantling (damaged planks should be
Performance data of the product in accordance with the sorted out in any case).
declaration of performance with respect to its essential Recycling solutions of the panels are not known in the moment.
characteristics according to EN But all panels can be used for energy recovery in specific
14041:2004+AC:2005+AC:2006. recovery facilities. A landfill of the material is not known.
Base materials/Ancillary materials
The composition of a Vinyl floor covering in mass % is: Disposal
• 64 % High Density Fibre board (HDF) The European waste code is 17 02 03 (plastics).
• 31 % PVC If repeated use as floor coverings is no longer possible, the
• 3 % Cork product can be sent for energy recovery to generate heat and
• 2 % Adhesives electricity.
HDF (high-density fibreboard) Open burning in a chimney is not possible, as the combustion
The core board is a HDF board composed of wood fibres and a of plastics leads to harmful emissions. Incineration should take
thermosetting resin, mainly MUF (melamine-urea- place in a plant with a connected flue gas cleaning system,
formaldehyde) resin. such as a waste incineration plant.
PVC based surface layer The surface layer consists of a Dispose of in any case accordance with Federal, State and
transparent wear layer and a decorative layer. Local Waste Disposal Regulations.
Balance layer
The balance layer can consist of different material e.g. cork.
2 Environmental Product Declaration - MMFA (Multilayer Modular Flooring Association) - Vinyl- HDF- floor covering
LCA: Calculation rules
values for the product stage (A1-A3), delivery (A4) and end of
Declared Unit life (C, D) have to be multiplied with the amount of waste (e.g.
Declared is 1 m2 Vinyl- HDF- floor covering with the 3% installation waste, factor 1.03).
specifications listed in the table below.
Module B2 is including provision of cleaning agent, energy and
Name Value Unit water consumption for the cleaning of the floor covering incl.
Declared unit 1 m2 wastewater treatment. The LCA results in this EPD are
declared for a one-year usage.
Grammage 9.11 kg/m2
Layer thickness 0.0095 m Module C1 considers manual deconstruction/ dismantling.
Gross density 944 kg/m3
Module C2 includes transportation of post-consumer waste to a
The EPD declares an average of a specific product from
waste processing plant (50km - truck diesel Euro 6).
factories of several manufacturers of floor coverings. The
averaging was done by weighting according to the total
Module C3: 100% Incineration in a waste incineration plant in
production quantities of the manufacturers. The EPD is
EU. The collection rate is set to 100%.
representative for the association MMFA. Regarding the
variability of production data of the individual manufacturers,
Module C4: As the product is incinerated at its end-of-life, this
slight fluctuations can occur due to different production
module is not relevant for this study and therefore not declared.
technologies, supply-chains and locations.
Module D includes potential benefits from all net flows given in
modules A5 and C3 that leave the product boundary system
System boundary after having passed the end-of-waste state in the form of
recovery potential.
Type of EPD: cradle to gate with options, modules A4, A5, B2,
modules C1–C3, module D.
Geographic Representativeness
Land or region, in which the declared product system is
Modules A1-A3 include processes that provide materials and
manufactured, used or handled at the end of the product´s
energy input for the system, manufacturing and transport
lifespan: Europe
processes up to the factory gate, as well as waste processing.
Module A4 includes transport of the floor covering to the place Comparability
of installation (100km - truck diesel Euro 6). Basically, a comparison or an evaluation of EPD data is only
possible if all the data sets to be compared were created
Module A5 includes the incineration of packaging material. according to EN 15804 and the building context, respectively
Installation efforts in form of offcuts or auxiliaries are not the product-specific characteristics of performance, are taken
declared in the EPD. into account. The used database is LCA FE (GaBi) 2023,
For a simplified calculation of the environmental impact of 1 m² version 2023.1.
flooring including a certain amount of installation offcuts the
LCA: Scenarios and additional technical information
Maintenance (B2) per year
Characteristic product properties of biogenic carbon
Name Value Unit
Water consumption 0.0068 m3
Information on describing the biogenic carbon content at
factory gate Auxiliary (Detergent) 0.051 kg
Name ValueUnit Electricity consumption 0.0739 kWh
kg
Biogenic carbon content in product 2.719
C
End of Life (C1-C3)
Biogenic carbon content in accompanying kg
0.086 Name Value Unit
packaging C
Collected separately waste type 9.11 kg
Waste materials for energy recovery 9,11 kg
Note: 1 kg of biogenic carbon is equivalent to 44/12 kg of CO .
2
Reuse, recovery and/or recycling potentials (D), relevant
scenario information
In module D, potential benefits from incineration processes in
module A3, A5 and C3 are declared.
Transport to the construction site (A4)
Name Value Unit
Litres of fuel 0.03 l/100km
Transport distance 100 km
Capacity utilisation (including empty runs) 55 %
3 Environmental Product Declaration - MMFA (Multilayer Modular Flooring Association) - Vinyl- HDF- floor covering
LCA: Results
The following tables display the LCA-results for 1 m² Vinyl- HDF- floor covering with a total thickness of 9.5 mm and a surface weight of
9.11 kg/m². LCA-results for module B2 declare a one-year usage.
The LCA-results are representative for MMFA Vinyl- HDF- floor coverings with the described product characteristics, including product
composition and geographical scope, and a thickness within the range of the collected data (9.1 - 10 mm).
DESCRIPTION OF THE SYSTEM BOUNDARY (X = INCLUDED IN LCA; MND = MODULE OR INDICATOR NOT DECLARED; MNR
= MODULE NOT RELEVANT)
Benefits and
Construction loads beyond
Product stage Use stage End of life stage
process stage the system
boundaries
la ire ta m w a Ry lp p u s tro p s n a rT g n iru tc a fu n a M e h t m o rf tro p s n a rTe tis e h t o t e ta g y lb m e s s A e s U e c n a n e tn ia M ria p e R tn e m e c a lp e R tn e m h s ib ru fe R y g re n e la n o ita re p Oe s u re ta w la n o ita re p Oe s u n o itc u rts n o c -e Dn o itilo m e d tro p s n a rT g n is s e c o rp e ts a W la s o p s iD -e s u e R-y re v o c e R-g n ilc y c e Rla itn e to p
A1 A2 A3 A4 A5 B1 B2 B3 B4 B5 B6 B7 C1 C2 C3 C4 D
X X X X X MND X MNR MNR MNR MND MND X X X MND X
RESULTS OF THE LCA - ENVIRONMENTAL IMPACT according to EN 15804+A2: 1 m² Vinyl- HDF- floor covering
Parameter Unit A1-A3 A4 A5 B2 C1 C2 C3 D
GWP-total kg CO 2 eq 5.73E+00 9.19E-02 3.42E-01 8.1E-02 0 3.9E-02 1.54E+01 -4.37E+00
GWP-fossil kg CO 2 eq 1.56E+01 8.79E-02 4.84E-02 7.72E-02 0 3.73E-02 5.43E+00 -4.35E+00
GWP-biogenic kg CO 2 eq -9.82E+00 4.02E-03 2.94E-01 3.74E-03 0 1.7E-03 9.97E+00 -2.31E-02
GWP-luluc kg CO 2 eq 9.84E-03 1.8E-06 2.06E-06 6.43E-06 0 7.61E-07 9.89E-04 -2.67E-04
ODP kg CFC11 eq 5.73E-11 6.8E-15 4.07E-14 3.66E-13 0 2.88E-15 4.92E-12 -3.07E-11
AP mol H+ eq 4.28E-02 1.02E-04 6.73E-05 1.15E-04 0 4.53E-05 7.2E-03 -5.11E-03
EP-freshwater kg P eq 3.47E-05 1.91E-08 1.18E-08 4.41E-06 0 8.1E-09 1.97E-06 -6.35E-06
EP-marine kg N eq 1.3E-02 3.71E-05 2.17E-05 5.08E-05 0 1.69E-05 3.13E-03 -1.53E-03
EP-terrestrial mol N eq 1.26E-01 4.21E-04 2.94E-04 3.75E-04 0 1.91E-04 3.78E-02 -1.64E-02
kg NMVOC
POCP 3.49E-02 9.64E-05 5.86E-05 1.4E-04 0 4.3E-05 8.07E-03 -4.28E-03
eq
ADPE kg Sb eq 1.88E-06 9.49E-10 3.74E-10 6.01E-09 0 4.02E-10 4.66E-08 -2.85E-07
ADPF MJ 2.31E+02 1.27E+00 1.02E-01 1.78E+00 0 5.37E-01 1.04E+01 -7.85E+01
m3 world eq
WDP 2.56E+00 1.61E-04 3.86E-02 1.36E-02 0 6.8E-05 1.66E+00 -3.72E-01
deprived
GWP = Global warming potential; ODP = Depletion potential of the stratospheric ozone layer; AP = Acidification potential of land and water; EP =
Eutrophication potential; POCP = Formation potential of tropospheric ozone photochemical oxidants; ADPE = Abiotic depletion potential for non-fossil
resources; ADPF = Abiotic depletion potential for fossil resources; WDP = Water (user) deprivation potential)
RESULTS OF THE LCA - INDICATORS TO DESCRIBE RESOURCE USE according to EN 15804+A2: 1 m² Vinyl- HDF- floor
covering
Parameter Unit A1-A3 A4 A5 B2 C1 C2 C3 D
PERE MJ 6.15E+01 5.34E-03 3.53E+00 1.39E-01 0 2.26E-03 1.03E+02 -2.1E+01
PERM MJ 1.04E+02 0 -3.5E+00 0 0 0 -1E+02 0
PERT MJ 1.65E+02 5.34E-03 2.49E-02 1.39E-01 0 2.26E-03 2.78E+00 -2.1E+01
PENRE MJ 1.93E+02 1.27E+00 4.87E-01 1.8E+00 0 5.39E-01 4.89E+01 -7.86E+01
PENRM MJ 3.9E+01 0 -3.86E-01 0 0 0 -3.86E+01 0
PENRT MJ 2.32E+02 1.27E+00 1.02E-01 1.8E+00 0 5.39E-01 1.04E+01 -7.86E+01
SM kg 0 0 0 0 0 0 0 0
RSF MJ 0 0 0 0 0 0 0 0
NRSF MJ 0 0 0 0 0 0 0 0
FW m3 7.72E-02 6.95E-06 9.09E-04 4.7E-04 0 2.94E-06 3.99E-02 -1.7E-02
PERE = Use of renewable primary energy excluding renewable primary energy resources used as raw materials; PERM = Use of renewable primary
energy resources used as raw materials; PERT = Total use of renewable primary energy resources; PENRE = Use of non-renewable primary energy
excluding non-renewable primary energy resources used as raw materials; PENRM = Use of non-renewable primary energy resources used as raw
materials; PENRT = Total use of non-renewable primary energy resources; SM = Use of secondary material; RSF = Use of renewable secondary fuels;
NRSF = Use of non-renewable secondary fuels; FW = Use of net fresh water
RESULTS OF THE LCA – WASTE CATEGORIES AND OUTPUT FLOWS according to EN 15804+A2:
1 m² Vinyl- HDF- floor covering
Parameter Unit A1-A3 A4 A5 B2 C1 C2 C3 D
HWD kg 3.45E-06 3.07E-12 2.35E-12 8.69E-11 0 1.3E-12 1.27E-10 -5E-09
NHWD kg 3.31E-01 1.16E-04 1.11E-02 7.12E-03 0 4.9E-05 1.88E+00 -3.73E-02
RWD kg 6.86E-03 1.44E-06 5.23E-06 1.22E-04 0 6.1E-07 4.29E-04 -5.56E-03
CRU kg 0 0 0 0 0 0 0 0
MFR kg 0 0 0 0 0 0 0 0
4 Environmental Product Declaration - MMFA (Multilayer Modular Flooring Association) - Vinyl- HDF- floor covering
MER kg 0 0 0 0 0 0 0 0
EEE MJ 1.15E+00 0 5.09E-01 0 0 0 1.68E+01 0
EET MJ 2.37E+00 0 9.17E-01 0 0 0 3.6E+01 0
HWD = Hazardous waste disposed; NHWD = Non-hazardous waste disposed; RWD = Radioactive waste disposed; CRU = Components for re-use;
MFR = Materials for recycling; MER = Materials for energy recovery; EEE = Exported electrical energy; EET = Exported thermal energy
RESULTS OF THE LCA – additional impact categories according to EN 15804+A2-optional:
1 m² Vinyl- HDF- floor covering
Parameter Unit A1-A3 A4 A5 B2 C1 C2 C3 D
Disease
PM 6.8E-07 6.31E-10 4.41E-10 9.78E-10 0 3.42E-10 4.05E-08 -4.34E-08
incidence
IR kBq U235 eq 9.25E-01 2.05E-04 8.18E-04 1.76E-02 0 8.67E-05 6.05E-02 -9.24E-01
ETP-fw CTUe 7.83E+01 8.88E-01 5.04E-02 1.13E+00 0 3.76E-01 5.55E+00 -1.58E+01
HTP-c CTUh 5.42E-08 1.64E-11 3.57E-12 3.13E-11 0 6.93E-12 3.29E-10 -8.47E-10
HTP-nc CTUh 1.46E-07 6.74E-10 2.32E-10 2.49E-09 0 2.85E-10 2.59E-08 -2.69E-08
SQP SQP 4.59E+02 4.04E-03 2.92E-02 1.19E-01 0 1.71E-03 2.96E+00 -1.38E+01
PM = Potential incidence of disease due to PM emissions; IR = Potential Human exposure efficiency relative to U235; ETP-fw = Potential comparative
Toxic Unit for ecosystems; HTP-c = Potential comparative Toxic Unit for humans (cancerogenic); HTP-nc = Potential comparative Toxic Unit for humans
(not cancerogenic); SQP = Potential soil quality index
Disclaimer 1 – for the indicator “Potential Human exposure efficiency relative to U235”. This impact category deals mainly with the
eventual impact of low-dose ionizing radiation on human health of the nuclear fuel cycle. It does not consider effects due to possible
nuclear accidents, occupational exposure or radioactive waste disposal in underground facilities. Potential ionizing radiation from the
soil, radon and from some construction materials is also not measured by this indicator.
Disclaimer 2 – for the indicators “abiotic depletion potential for non-fossil resources”, “abiotic depletion potential for fossil resources”,
“water (user) deprivation potential, deprivation-weighted water consumption”, “potential comparative toxic unit for ecosystems”,
“potential comparative toxic unit for humans – cancerogenic”, “Potential comparative toxic unit for humans - not cancerogenic”,
“potential soil quality index”. The results of this environmental impact indicator shall be used with care as the uncertainties on these
results are high as there is limited experience with the indicator.
References
Standards procedures.
EN ISO 10874 Further References
EN ISO 10874:2012 + A1:2020, Resilient, textile and laminate
floor coverings - Classification. BNB
BBSR table (german): 'Nutzungsdauern von Bauteilen zur
EN 13501-1 Lebenszyklusanalyse nach BNB', Bundesinstitut für Bau-,
Stadt- und Raumforschung, Referat II Nachhaltiges Bauen;
EN 13501-1:2019-01-14;Fire classification of construction online available under:
products and building elements. https://www.nachhaltigesbauen.de/austausch/nutzungsdauern-
von-bauteilen/, 2017.
EN 14041
EN 14041:2004+AC:2005+AC:2006, Resilient, textile IBU 2021
and laminate floor coverings – Essential characteristics. Institut Bauen und Umwelt e.V.: General Instructions for the
EPD programme of Institut Bauen und Umwelt e.V., Version
EN 15804 2.0, Berlin: Institut Bauen und Umwelt e.V., https://ibu-
EN 15804:2012+A1 2013, Sustainability of construction works epd.com/, 2021.
— Environmental Product Declarations — Core rules for the
product category of construction products. IBU PCR Part A
PCR - Part A: Calculation Rules for the Life Cycle Assessment
EN 15804 and Requirements on the Project Report according to EN
EN 15804:2012+A2:2019+AC:2021, Sustainability of 15804+A2:2019, version 1.3, Institut Bauen und Umwelt e.V.,
construction works — Environmental Product Declarations — https://ibu-epd.com/, 2022.
Core rules for the product category of construction products.
IBU PCR Part B
EN 16511 PCR – Part B: Requirements of the EPD for floor coverings,
EN 16511:2023; Modular mechanical locked floor coverings version 16/09/2022, Institut Bauen und Umwelt e.V., https://ibu-
(MMF) – Specification, requirements and test method for epd.com/, 2022.
multilayer modular panels for floating installation.
LCAfE software and MLC databases
EN ISO 20326 LCAfE and MLC databases (f.k.a. GaBi) by Sphera. Version
EN ISO 20326:2018 + A1:2020, Resilient floor coverings – CUP 2023.1. Sphera Solutions GmbH,
Specification for floor panels/assembly for loose laying. https://sphera.com/product-sustainability-gabi-data-search/,
2023.
ISO 14025
EN ISO 14025:2011, Environmental labels and declarations —
Type III environmental declarations — Principles and
5 Environmental Product Declaration - MMFA (Multilayer Modular Flooring Association) - Vinyl- HDF- floor covering
Publisher
Institut Bauen und Umwelt e.V. +49 (0)30 3087748- 0
Hegelplatz 1 info@ibu-epd.com
10117 Berlin www.ibu-epd.com
Germany
Programme holder
Institut Bauen und Umwelt e.V. +49 (0)30 3087748- 0
Hegelplatz 1 info@ibu-epd.com
10117 Berlin www.ibu-epd.com
Germany
Author of the Life Cycle Assessment
Sphera Solutions GmbH +49 711 341817-0
Hauptstraße 111- 113 info@sphera.com
70771 Leinfelden-Echterdingen www.sphera.com
Germany
Owner of the Declaration
MMFA - Multilayer Modular Flooring Association +32 2 788 3169
Mittelstrasse 50 info@mmfa.eu
33602 Bielefeld www.mmfa.eu
Germany
6 Environmental Product Declaration - MMFA (Multilayer Modular Flooring Association) - Vinyl- HDF- floor covering
