ENVIRONMENTAL PRODUCT DECLARATION
as per ISO 14025 and EN 15804+A2
Owner of the Declaration KE Fibertec AS
Publisher Institut Bauen und Umwelt e.V. (IBU)
Programme holder Institut Bauen und Umwelt e.V. (IBU)
Declaration number EPD-KEF-20230264-CBI1-EN
Issue date 21.12.2023
Valid to 20.12.2028
MultiWeave textile-based ventilation duct
KE Fibertec AS
www.ibu-epd.com | https://epd-online.com
General Information
KE Fibertec AS MultiWeave textile-based ventilation duct
Programme holder Owner of the declaration
IBU – Institut Bauen und Umwelt e.V. KE Fibertec AS
Hegelplatz 1 Industrivej Vest 21
10117 Berlin 6600 Vejen
Germany Denmark
Declaration number Declared product / declared unit
EPD-KEF-20230264-CBI1-EN 1 kg of MultiWeave ventilation duct including mounting equipment.
This declaration is based on the product category rules: Scope:
Ventilation ducts, 01.08.2021 This is a representative EPD describing the production of 1 kg KE Fibertec
(PCR checked and approved by the SVR) AS custom-made textile-based ventilation ducts of the MultiWeave (MW)
line including mounting equipment. KE Fibertec AS have two production
sites. One in Vejen in Denmark, which includes both a weaving mill, laser
Issue date cutting and sewing room. The other production site is located in the Czech
Republic and includes laser cutting and a sewing room. Both sites are
21.12.2023
included in the results of this EPD.
The main component of the textile duct is polyester and the mounting
Valid to
equipment is made of aluminium. The data represents the production of
20.12.2028 2021.
The owner of the declaration shall be liable for the underlying information
and evidence; the IBU shall not be liable with respect to manufacturer
information, life cycle assessment data and evidences.
The EPD was created according to the specifications of EN 15804+A2. In
the following, the standard will be simplified as EN 15804.
Verification
The standard EN 15804 serves as the core PCR
Independent verification of the declaration and data according to ISO
14025:2011
Dipl.-Ing. Hans Peters
(Chairman of Institut Bauen und Umwelt e.V.) internally X externally
Florian Pronold Ms Jane Anderson,
(Managing Director Institut Bauen und Umwelt e.V.) (Independent verifier)
1 Environmental Product Declaration - KE Fibertec AS - MultiWeave textile-based ventilation duct
Product
• DS 428
Product description/Product definition • EN 13501-1
This is a representative EPD representing the MultiWeave Aluminium rail:
product group. The textile ducts made by KE Fibertec A/S are
• BS EN 573-3:2019+A1
either round, semi-round or quarter-round ducts made of a light
• EN 515
weight textile material. They are designed for delivery and
• DIN EN 10204 2.2
distribution of cooled or heated air. The textile is suitable for
ventilation purposes in schools, offices, shops, showrooms Technical data
production facilities and food industry, and other types of Name Value Unit
rooms. The textile ducts primarily consist of two parts. One
Material textile duct Polyester -
being the textile tube and the other the mounting equipment
Material used for mounting Aluminium -
consisting of an aluminium rail. The textile used is
Meter weight Duct incl. mounting material 1 - 3 kg/m
manufactured at KE Fibertec's own weaving mill and is
designed for air distribution. The mounting equipment is made Operating Temperature (max. permitted) 80 °C
of aluminium. Textile ducts can be equipped with nozzles to Operating Temperature (min. permitted) -45 °C
enhance good ventilation in large rooms.
Performance data of the product with respect to its
characteristics in accordance with the relevant technical
The production of KE Fibertec's textile-based ventilation ducts
provision (no CE-marking).
have so far not been subject to EU harmonisation legislation.
Hence, for the use and application of the products the Base materials/Ancillary materials
respective national provisions at the place of use apply.
Name Value Unit
Application Textile Polyester 37 %
KE Fibertecs MultiWeave textile-based ventilations ducts are Aluminium Mounting equipment 54 %
custom-made to provide the optimal service in the specific room Ancillary materials 9 %
and under the specific conditions they are placed in. The
This product/article/at least one partial article contains
ventilation ducts are made for blowing in and distributing air.
substances listed in the candidate list (date: 15.05.2023)
Technical Data exceeding 0.1 percentage by mass: No
The main components - polyester and aluminium - of the
Reference service life
ventilation duct covered by this EPD are tested in accordance
No reference service life is declared since the complete use
with the following standards.
stage is not included. However, the expected lifetime of the
Polyester:
product is 25 years. Some of the ventilation ducts are over 35
• ISO 9001
years and still in service. The lifetime of the product depends on
• EN 779
the operation conditions and maintenance of the product.
• ISO 14644-1
• ISO 13937-2
LCA: Calculation rules
Declared unit
Declared Unit
The declared unit is 1 kg of MultiWeave ventilation duct Name Value Unit
including mounting equipment. This study describes the Declared unit 1 kg
environmental impacts of a representative textile-based Mass reference 1 - 3 kg/rm
ventilation duct of the MultiWeave line manufactured at KE
Raw density Polyester 500 kg/m3
Fibertec. The input material represents a weighted average for
all the products under the given product group. The data is This is a representative EPD representing an average
based on the production in 2021 and the total production Multiweave ventilation duct as these are always costum made.
volume of the same period. The processing at the production The representative product is compiles based on 5 cases. The
site is almost identical for the different products. The only main components of the ventilation duct are the aluminium rail
difference is the amount of clipping and the addition of nozzles for mounting and the polyester. The smaller the ducts (length
for one type of ventilation duct. An average amount of clippings and diameter) the higher the share of aluminium. The standard
is applied in this study and an amount of nozzle is added in the variation within the aluminium and polyester input is 4 and 5 %,
modelling. respectively. This means that the environmental impact of
smaller ventilation ducts where the share of aluminium is higher
This EPD represents the MultiWeave product group. The the environmental impact will be higher compared to larger
differences within the MultiWeave ventilation ducts are the ventilation ducts where the share of aluminium will be smaller.
dimensions and permeability of the fabric. However, the
System boundary
production processes of the products within the MultiWeave line
are the same. Therefore, a representative EPD is made to This is a cradle-to-gate EPD - with options, including the
cover this product group. The representative product is modules A1-A3, B2, C1-4 and D.
compiled by using 5 solutions varying in size and calculating a
weighted average of each component of the ventilation duct. Production stage - Modules A1-3
The production stage includes:
• A1, raw material extraction and processing, processing
of secondary material from previous product systems,
2 Environmental Product Declaration - KE Fibertec AS - MultiWeave textile-based ventilation duct
when applicable. packaging material is not included as module A5 is not
• A2, transport to factory gate and internal transport declared.
• A3, manufacturing of products and packaging, as well KE Fibertec have due to their cradle-to-cradle certification focus
as assembly and processing up to the end-of-waste on recyclability of their produkt. KE Fibertec has established a
state. takeback scheme to increase the amount of recycled material in
All of the above-mentioned are included in this study. Wastes their products. Hence, most of the material is send to recycling
and losses of the manufacturing processes are included in the within their take back scheme. The waste processes in C3
processes in which they occur according to the polluter pays include the sorting of aluminium, polyester, POM, nylon, and
principle. The construction of the manufacturing facility is not steel. The following sorting efficiencies have been used:
taken into account.
Aluminium - 98 % recycling and 2 % landfill
For the environmental impact, the use of green electricity was Polyester - 91.3 % recycling and 8.7 % incineration with energy
calculated taking into account the residual electricity mix for the recovery
remaining electricity. The proportion of the electricity demand POM - 90.5 % recycling and 9.5 % incineration with energy
covered by green electricity in the total electricity demand in A3 recovery
is 90 %. Steel - 96 % recycling and 4 % landfill
Other - 100 % recycling
Use stage - Module B2 maintenance
The use stage includes: C3 also includes the incineration of the above mentioned
materials as well as regranulation of the polyester. After this all
• B2, maintenance
the material have entered the end-of-waste stage.
The permeability of the textile ducts will decrease over time due
to depositions of dust and particles. Therefore, the ducts need
Benefits and loads beyond the system boundaries -
to be washed regularly. KE Fibertec provides a washing service
Module D
for their customers. The customer sends the ducts to KE
The benefits and loads include:
Fibertec, who will then wash the ducts and deliver them back to
the customer. The washing service included in this study • D, potential benefits from reuse, recycling and recovery
includes transport, the use of water, electricity, detergent as outside the scope of the study
well as the washing machine itself. The transport distance is not • D, potential loads related to processing to reach
known and was assumed to be 300 km. The 300 km from the equivalent materials to virgin input material
production site in Vejen in Denmark will cover the entire territory In this EPD, the recycling of the main components - fabric and
of Denmark. The washing service is primarily used by aluminium is credited. Credit is only given to the net production
customers located relatively close to Vejen as the service of primary material. Steel and polyoxymethylene (POM) from
should be viable. A sensitivity test was made for the transport small mounting materials and nozzles are also credited in this
distance by changing the distance to 600 km and the result module. Also, here the amount of secondary material is
showed, that it did not change the overall conclusion. considered, and credit is only given to the avoidance of primary
B2 is calculated based on 1 washing cycle. The amount of material. As described above module D includes the loads and
cycles during the lifetime of the ventilation duct varies between benefits beyond system boundaries. To account for the loads
application type. They are maximum washed 2 times every year required to achieve functional equivalence to the input material
and minimum once every 10 years. On average the ventilation the processing of remelting aluminium and processing of fabric
ducts are washed 1 time per year. is accounted for. The same applies to the small fractions of
This EPD entails 2 B2 scenarios. B2 and B2/1. steel. Since a small fraction of plastic products such as
B2 is a reference scenario using a European electricity mix polyester and nylon is incinerated heat and electricity are
B2/1 is using Danish wind power representing the washing recovered and a credit for this is given in this module.
service provided by KE Fibertec.
Geographic Representativeness
End-of-life stage - Modules C1-C4 Land or region, in which the declared product system is
The end-of-life stage includes: manufactured, used or handled at the end of the product´s
C1, deconstruction and demolition lifespan: Denmark
• C2, transport to waste processing
• C3, waste processing for reuse, recovery and/or Comparability
recycling
Basically, a comparison or an evaluation of EPD data is only
• C4, disposal
possible if all the data sets to be compared were created
The deconstruction of the products is assumed to be done
according to EN 15804 and the building context, respectively
manually. As a result, no processes have been added to
the product-specific characteristics of performance, are taken
module C1. The ventilation ducts are sold on the global market.
into account. The system model EN15804 - cut-off available in
This means that transportation distance, technology and waste
the LCI database Ecoinvent v. 3.9 is used in this EPD
processing are modelled accordingly. End-of-life treatment of
LCA: Scenarios and additional technical information
Information on describing the biogenic carbon content at
Characteristic product properties of biogenic carbon
factory gate
The biogenic carbon content quantifies the amount of biogenic
carbon in a construction product leaving the factory gate. Both Name ValueUnit
the biogenic content of the product and the accompanying kg
Biogenic carbon content in product -
packaging are declared. C
Biogenic carbon content in accompanying kg
0.035
Note: 1 kg of biogenic carbon is equivalent to 44/12 kg of CO 2. packaging Cardboard C
3 Environmental Product Declaration - KE Fibertec AS - MultiWeave textile-based ventilation duct
of KE Fibertecs Cradle-to-cradle certifikation.
The following technical scenario information can be used for Name Value Unit
the declared modules and optional modules for non-declared
Collected separately waste type 1 kg
modules. The following technical scenario information covers
Polyester 0.40 kg
the disposal of the accompanying packaging material,
produced in module A3, on the construction site as module A5 Aluminium 0.54 kg
is not declared in this EPD, B2 maintenance, end-of-life and POM 0.03 kg
loads and benefits beyond the system boundaries. Steel 0.02 kg
Assembly (A5) Other material 0.01 kg
Name Value Unit Recycling Polyester 0.36 kg
Cardboard packaging for recycling 0.07 kg Recycling Aluminium 0.53 kg
Recycling POM 0.03 kg
Maintenance (B2)
Recycling Steel 0.02 kg
This module includes the washing service of KE Fibertec. A
Energy recovery Polyester 0.04 kg
sensitivity analysis was made on the transportation distance
and showed that doublling the distance does not change the Energy recovery POM 0.002 kg
overall conclusion of the EPD. Module B2 represents 1 the Energy recovery Other material 0.01 kg
input for 1 washing cycle and a ventilation ducts is an average Landfilling Aluminium 0.01 kg
washed once a year.
Landfilling Steel 0.001 kg
Two scenarios are made for the washing service. One using
Transport Sorting 200 km
European power mix as describes in PCR part 1 (B2/1) and one
representing KE Fibertec washing service at their facilities in Transport Recycling 100 km
Denmark. For the second scenario at KE Fibertecs facility Transport Incineration 100 km
transport is included (B2/2). Transport Landfil 150 km
Name Value Unit
Reuse, recovery and/or recycling potentials (D), relevant
Water consumption per cycle 0.24 m3
scenario information
Detergent per cycle 0.05 L
The following values in the table are amounts contributing to
Washing load per cycle 12 kg the loads and benefits included in module D.
Electricity consumption per cycle 0.15 kWh Name Value Unit
Transport distance 300 km Recycling of polyester From module C3 0.30 kg
Recycling of aluminium From module C3 0.14 kg
End of life (C1-C4)
Recycling of POM From module C3 0.03 kg
The following table shows the technical information scenario
regarding waste module C stating the different waste fractions Recycling of steel From module C3 0.0004 kg
and their collection form and waste processing steps. The Incineration of polyester From module C3 0.02 kg
transportation distances have been assumed as no data on Incineration of POM From module C3 0.002 kg
average distances to waste treatment facilities have been
Incineration of other material From module C3 0.01 kg
found. However, a sensitivity analysis was conducted doubling
the transportation distances. The test showed, that changing Credits are only given to the net amount leaving the product
the distances did not have a significant influence on the overall system that has passed the end-of-waste state. In the LCA
results and did not change the overall conclusion. calculation loads related to obtaining equivalent functions as
KE Fibertec has established a takeback scheme, hence a large the original virgin material are included as well as the benefits
part of the products are recycled. This has been done as a part of avoided production of the given virgin material.
4 Environmental Product Declaration - KE Fibertec AS - MultiWeave textile-based ventilation duct
LCA: Results
The following table shows the LCA results obtained in this study.
For calculation of the results, characterization was used on a model created of individual inputs from different LCIA methods to comply
with EN15804+A2 which is yet to be fully implemented in the SimaPro software. As a result, the LCIA has been calculated in Excel
using the following methods from EcoInvent v.3.9:
• EF v.3.1 EN 15804
• EN 15804 inventory indicators according to ISO 21930
The additional indicators are retrieved by using Ecoinvent cumulative LCIA results for the system model EN15804, cut-off. It follows
ISO 21930 for all the datasets; hence the results include all the background processes as well as foreground processes.
C1 is declared as 0 since manual deconstruction is assumed.
The estimated impact results are only relative statements which do not indicate the endpoints of the impact categories, exceeding
threshold values, safety margins or risks.
DESCRIPTION OF THE SYSTEM BOUNDARY (X = INCLUDED IN LCA; MND = MODULE OR INDICATOR NOT DECLARED; MNR
= MODULE NOT RELEVANT)
Benefits and
Construction loads beyond
Product stage Use stage End of life stage
process stage the system
boundaries
la ire ta m w a Ry lp p u s tro p s n a rT g n iru tc a fu n a M e h t m o rf tro p s n a rTe tis e h t o t e ta g y lb m e s s A e s U e c n a n e tn ia M ria p e R tn e m e c a lp e R tn e m h s ib ru fe R y g re n e la n o ita re p Oe s u re ta w la n o ita re p Oe s u n o itc u rts n o c -e Dn o itilo m e d tro p s n a rT g n is s e c o rp e ts a W la s o p s iD -e s u e R-y re v o c e R-g n ilc y c e Rla itn e to p
A1 A2 A3 A4 A5 B1 B2 B3 B4 B5 B6 B7 C1 C2 C3 C4 D
X X X MND MND MND X MNR MNR MNR MND MND X X X X X
RESULTS OF THE LCA - ENVIRONMENTAL IMPACT according to EN 15804+A2: 1 kg MultiWeave ventilation duct incl.
mounting equipment
Parameter Unit A1-A3 B2 B2/1 C1 C2 C3 C4 D
GWP-total kg CO 2 eq 6.1E+00 8.49E-01 7.71E-01 0 1.48E-01 6.9E-01 1.82E-04 -2.26E+00
GWP-fossil kg CO 2 eq 6.07E+00 8.71E-01 7.93E-01 0 1.48E-01 5.86E-01 1.68E-04 -2.23E+00
GWP-biogenic kg CO 2 eq 2.23E-02 0 0 0 1.29E-04 1.04E-01 1.42E-05 -3.39E-03
GWP-luluc kg CO 2 eq 3.07E-02 5.34E-02 5.34E-02 0 7.3E-05 4.15E-04 5.02E-08 -2.49E-02
ODP kg CFC11 eq 7.63E-06 1.7E-08 1.54E-08 0 3.22E-09 1.23E-08 4.45E-12 -4.59E-06
AP mol H+ eq 3.29E-02 2.8E-03 2.39E-03 0 3.23E-04 1.36E-03 1.1E-06 -1.34E-02
EP-freshwater kg P eq 2.16E-03 1.32E-04 9.34E-05 0 1.05E-05 1.43E-04 2.03E-08 -6.96E-04
EP-marine kg N eq 6.89E-03 1.16E-03 1.09E-03 0 8.2E-05 1.04E-03 4.49E-07 -1.93E-03
EP-terrestrial mol N eq 6.42E-02 7.15E-03 6.49E-03 0 8.28E-04 3.8E-03 4.9E-06 -1.96E-02
kg NMVOC
POCP 2.61E-02 3.34E-03 3.11E-03 0 5.01E-04 1.25E-03 1.73E-06 -7.43E-03
eq
ADPE kg Sb eq 6.38E-05 3.57E-06 3.52E-06 0 4.94E-07 2.4E-06 7.71E-10 2.29E-05
ADPF MJ 1.01E+02 1.37E+01 1.23E+01 0 2.11E+00 4.51E+00 3.56E-03 -3.93E+01
m3 world eq
WDP 5.62E+00 4.77E-01 4.61E-01 0 1.05E-02 1.13E-01 9.1E-05 -1.96E+00
deprived
GWP = Global warming potential; ODP = Depletion potential of the stratospheric ozone layer; AP = Acidification potential of land and water; EP =
Eutrophication potential; POCP = Formation potential of tropospheric ozone photochemical oxidants; ADPE = Abiotic depletion potential for non-fossil
resources; ADPF = Abiotic depletion potential for fossil resources; WDP = Water (user) deprivation potential)
RESULTS OF THE LCA - INDICATORS TO DESCRIBE RESOURCE USE according to EN 15804+A2: 1 kg MultiWeave ventilation
duct incl. mounting equipment
Parameter Unit A1-A3 B2 B2/1 C1 C2 C3 C4 D
PERE MJ 2.03E+01 2.19E+00 2.19E+00 0 3.3E-02 6.81E-01 6.26E-04 -6.55E+00
PERM MJ 0 0 0 0 0 0 0 0
PERT MJ 2.03E+01 2.19E+00 2.19E+00 0 3.3E-02 6.81E-01 6.26E-04 -6.55E+00
PENRE MJ 9.03E+01 1.38E+01 1.38E+01 0 2.12E+00 2.12E+00 3.56E-03 -3.09E+01
PENRM MJ 8.26E+00 0 0 0 0 -8.16E+00 0 0
PENRT MJ 9.85E+01 1.38E+01 1.38E+01 0 2.12E+00 -6.04E+00 3.56E-03 -3.09E+01
SM kg 2.5E-01 0 0 0 0 0 0 6.26E-01
RSF MJ 0 0 0 0 0 0 0 0
NRSF MJ 0 0 0 0 0 0 0 0
FW m3 1.3E-01 3.31E-02 3.2E-02 0 2.55E-04 2.97E-03 4.87E-06 -3.78E-02
PERE = Use of renewable primary energy excluding renewable primary energy resources used as raw materials; PERM = Use of renewable primary
energy resources used as raw materials; PERT = Total use of renewable primary energy resources; PENRE = Use of non-renewable primary energy
excluding non-renewable primary energy resources used as raw materials; PENRM = Use of non-renewable primary energy resources used as raw
materials; PENRT = Total use of non-renewable primary energy resources; SM = Use of secondary material; RSF = Use of renewable secondary fuels;
5 Environmental Product Declaration - KE Fibertec AS - MultiWeave textile-based ventilation duct
NRSF = Use of non-renewable secondary fuels; FW = Use of net fresh water
RESULTS OF THE LCA – WASTE CATEGORIES AND OUTPUT FLOWS according to EN 15804+A2:
1 kg MultiWeave ventilation duct incl. mounting equipment
Parameter Unit A1-A3 B2 B2/1 C1 C2 C3 C4 D
HWD kg 3.52E-01 1.65E-02 1.21E-02 0 1.44E-03 1.25E-02 1.42E-04 -1.38E-01
NHWD kg 9.03E+00 5.64E-01 3.78E-01 0 4.37E-02 7.66E-01 1.19E-02 -3.12E+00
RWD kg 4.72E-05 3.18E-06 1.43E-06 0 1.69E-07 4.82E-06 1.3E-09 -1.27E-05
CRU kg 0 0 0 0 0 0 0 0
MFR kg 9.2E-02 0 0 0 0 8.76E-01 0 0
MER kg 9.28E-06 0 0 0 0 8.9E-02 0 0
EEE MJ 0 0 0 0 0 3.02E-01 0 0
EET MJ 0 0 0 0 0 5.29E-01 0 0
HWD = Hazardous waste disposed; NHWD = Non-hazardous waste disposed; RWD = Radioactive waste disposed; CRU = Components for re-use;
MFR = Materials for recycling; MER = Materials for energy recovery; EEE = Exported electrical energy; EET = Exported thermal energy
RESULTS OF THE LCA – additional impact categories according to EN 15804+A2-optional:
1 kg MultiWeave ventilation duct incl. mounting equipment
Parameter Unit A1-A3 B2 B2/1 C1 C2 C3 C4 D
Disease
PM 3.11E-07 6.05E-08 5.88E-08 0 1.1E-08 1.24E-07 2.43E-11 -1.47E-07
incidence
IR kBq U235 eq 7.52E-01 5.45E-02 2.3E-02 0 2.84E-03 8.33E-02 2.96E-05 -1.84E-01
ETP-fw CTUe 3.76E+01 9.82E+00 9.66E+00 0 1.03E+00 1.8E+00 8.88E-02 2.33E+00
HTP-c CTUh 8.52E-09 7.25E-10 6.86E-10 0 7.04E-11 6.72E-10 3.21E-13 -3.87E-09
HTP-nc CTUh 1.04E-07 9.99E-09 9.38E-09 0 1.5E-09 5.55E-09 2.83E-12 -3.55E-08
SQP SQP 2.08E+01 1.14E+01 1.11E+01 0 1.27E+00 2.02E+00 7.01E-03 -2.17E+00
PM = Potential incidence of disease due to PM emissions; IR = Potential Human exposure efficiency relative to U235; ETP-fw = Potential comparative
Toxic Unit for ecosystems; HTP-c = Potential comparative Toxic Unit for humans (cancerogenic); HTP-nc = Potential comparative Toxic Unit for humans
(not cancerogenic); SQP = Potential soil quality index
Disclaimer 1 – for the indicator 'Potential Human exposure efficiency relative to U235'. This impact category deals mainly with the
eventual impact of low-dose ionizing radiation on human health of the nuclear fuel cycle. It does not consider effects due to possible
nuclear accidents, occupational exposure or radioactive waste disposal in underground facilities. Potential ionizing radiation from the
soil, radon and from some construction materials is also not measured by this indicator.
Disclaimer 2 – for the indicators 'abiotic depletion potential for non-fossil resources', 'abiotic depletion potential for fossil resources',
'water (user) deprivation potential, deprivation-weighted water consumption', 'potential comparative toxic unit for ecosystems', 'potential
comparative toxic unit for humans – cancerogenic', 'Potential comparative toxic unit for humans - not cancerogenic', 'potential soil
quality index'. The results of this environmental impact indicator shall be used with care as the uncertainties on these results are high
as there is limited experience with the indicator.
References
Standards
BS EN 573-3:2019+A1 EN 13501-1
BS EN 573-3:2019+A1:2022, Aluminium and aluminium alloys. EN 13501-1:2018, Fire classification of construction products
Chemical composition and form of wrought products Chemical and building elements – Part 1: Classification
composition and form of products using data from reaction to fire tests Fire class B-s1-d0
DIN EN 10204 2.2 ISO 13937-2
DIN EN 10204 2.2, Metallic products - Types of inspection ISO 13937-2:2000, Textiles — Tear properties of fabrics — Part
documents (non-specific inspections) 2: Determination of tear force of trouser-shaped test specimens
(Single tear method)
DS 428
DS 428:2019, Fire protection of ventilation systems ISO 14025
ISO 14025:2011, Environmental labels and declarations —
EN 515 Type III environmental declarations — Principles and
EN 515:2017, Aluminium and aluminium alloys - Wrought procedures.
products - Temper designations
ISO 14040
EN 779 ISO 14040:2006, Environmental management –Life cycle
EN 779:2012, Particulate air filters for general ventilation – assessment - Principles and framework; English version
Determination of the filtration performance
ISO 14044
ISO 9001 ISO 14044:2006, Environment Management – LifeCycle
ISO 9001:2015, Quality management systems – Requirements Assessment – Requirements and Instructions; English version
EN ISO 14044:2006.
EN 15804
EN 15804 EN 15804:2012+A2:2019+AC:2021, Sustainability of ISO 14644-1
construction works — Environmental Product Declarations — ISO 14644-1:2015, Cleanrooms and associated controlled
Core rules for the product category of construction products. environments — Part 1: Classification of air cleanliness by
6 Environmental Product Declaration - KE Fibertec AS - MultiWeave textile-based ventilation duct
particle concentration B., Reinhard, J., Moreno-Ruiz, E., and Weidema, B., 2016. The
ecoinvent database version 3 (part pp.1218–1230. [Accessed
ISO 21930 25-05-2023]
ISO 21930:2017, Sustainability in buildings and civil
engineering works — Core rules for environmental IBU 2021
product declarations of construction products and services Product Category Rules for Building-Related Products
and Services, Part A: Calculation Rules for the Life
Further References Cycle Assessment and Requirements on the Project
ECHA candidate list Report, Version 1.3
Candidate List of substances of very high concern for
Authorisation IBU 2023
https://echa.europa.eu/candidate-list-table [Accessed 25-05- PCR Guidance-Text for Building-Related Products and
2023] Services, Part B: Requirements on the EPD for Ventilation
ducts, Version 1.0
EcoInvent 3.9
EcoInvent database version 3.9, cut-off, EN15804model. LCIA SimaPro 2023
methodology EF v3.1 EN15804.Wernet, G., Baue,., Steubing, LCA software SimaPro version 9.5.
7 Environmental Product Declaration - KE Fibertec AS - MultiWeave textile-based ventilation duct
Publisher
Institut Bauen und Umwelt e.V. +49 (0)30 3087748- 0
Hegelplatz 1 info@ibu-epd.com
10117 Berlin www.ibu-epd.com
Germany
Programme holder
Institut Bauen und Umwelt e.V. +49 (0)30 3087748- 0
Hegelplatz 1 info@ibu-epd.com
10117 Berlin www.ibu-epd.com
Germany
Author of the Life Cycle Assessment
Viegand Maagøe +45 33349000
Nørre Farimagsgade 37 info@viegandmaagoe.dk
1364 København K viegandmaagoe.dk
Denmark
Owner of the Declaration
KE Fibertec AS +4575364200
Industrivej Vest 21 info@ke-fibertec.dk
6600 Vejen www.ke-fibertec.com/da/
Denmark
8 Environmental Product Declaration - KE Fibertec AS - MultiWeave textile-based ventilation duct
