ENVIRONMENTAL-PRODUCT DECLARATION
as per ISO 14025 and EN 15804+A2
Owner of the Declaration European Producers of Laminate Flooring (EPLF®)
Publisher Institut Bauen und Umwelt e.V. (IBU)
Programme holder Institut Bauen und Umwelt e.V. (IBU)
Declaration number EPD-EPL-20210138-CBE2-EN
Issue date 09.07.2021
Valid to 08.07.2026
DPL laminate flooring
European Producers of Laminate Flooring e.V.
www.ibu-epd.com | https://epd-online.com
General Information
European Producers of Laminate Flooring DPL laminate flooring
e.V.
Programme holder Owner of the declaration
IBU – Institut Bauen und Umwelt e.V. European Producers of Laminate Flooring (EPLF®)
Hegelplatz 1 Mittelstraße 50
10117 Berlin 33602 Bielefeld
Germany Germany
Declaration number Declared product / declared unit
EPD-EPL-20210138-CBE2-EN 1m² of DPL floor covering
This declaration is based on the product category rules: Scope:
Floor coverings, 01.08.2021 This Environmental Product Declaration refers to a representative
(PCR checked and approved by the SVR) European DPL floor covering produced by manufacturers that are
members of EPLF®. Data are based upon production during 2019 in
Europe.
Issue date
The laminate floor covering described in this EPD has a thickness of 8 mm
09.07.2021
and meets the requirements
of the use classes: 21-23, 31-34 according to EN 13329, EN ISO 10874. In
order to enable the
Valid to
user of the EPD to calculate the LCA results for different thicknesses and
08.07.2026 use
classes, the EPD contains the respective calculation rules.
The owner of the declaration shall be liable for the underlying information
and evidence; the IBU shall not be liable with respect to manufacturer
information, life cycle assessment data and evidences.
The EPD was created according to the specifications of EN 15804+A2. In
the following, the standard will be simplified as EN 15804 bezeichnet.
Verification
The standard EN 15804 serves as the core PCR
Independent verification of the declaration and data according to ISO
Dipl.-Ing Hans Peters
14025:2011
(chairman of Institut Bauen und Umwelt e.V.)
internally X externally
Florian Pronold Matthias Klingler,
(Managing Director Institut Bauen und Umwelt e.V.) (Independent verifier)
1 Environmental-Product Declaration - European Producers of Laminate Flooring e.V. - DPL laminate flooring
Product
The composition of a DPL floor covering in mass % is:
Product description/Product definition
• 90-95 % High Density Fibre board (HDF)
DPL floor coverings described in this EPD are produced by
• 1-3 % paper
member companies of EPLF®. The floor coverings meet the
• 4-7 % resin
requirements of EN 13329.
• <1 % corundum
DPL floorings consist of a number of layers. On the top side
there is a decor with a transparent, wear-resistant contact
surface; in the middle there is a core layer made of high-density
wood fibres and on the back side there is a stabilizing layer to
HDF (high-density fibreboard)
guarantee floor stability. The decorative paper of a DPL floor
covering can be printed with any design and gives the floor its
individual appearance.
According to EPLF the participating companies
The core board is an HDF board composed
are representative for the declaration of the product, the
of wood fibres and a thermosetting resin, mainly MUF
weighting was done
(melamine-urea-formaldehyde) resin.
according to production volumes. For the placing on the
market of the product in the European Union/European Free
Trade
Association (EU/EFTA) (with the exception of Switzerland)
Paper
Regulation
(EU) No. 305/2011 (CPR) applies. The product needs a
declaration of
performance taking into consideration EN 13329 and the
The renewable resource wood is the main
CE-marking. For the application and use the respective national
raw material for paper production.
provisions apply.
Application
The laminate floor covering described in this EPD is intended to
Resins
be used within a building and meets the requirements of the
use classes: 21-23, 31-34 according to EN 13329, EN ISO
10874.
The used amino resins are
For the application and use
melamine-urea-formaldehyde resins. Amino resins are
the respective national provisions apply.
thermosetting resins that
Technical Data are cured using heat and pressure.
The technical specifications of the products within the scope of
the EPD shall be listed, including the reference to the test
methods/test standards for each specification.
Corundum
For products with CE marking, the technical specifications must
be specified in accordance with information in the declaration of
performance. The properties relevant to the product should be
specified in the table below. If no information is given for
properties, an explanation must be given in the background Bauxite is the mineral resource of
report to the EPD as to why the property is not relevant to the corundum. By using aluminiumoxide (Al 2O 3) the surface layer
product. of a laminate flooring obtains abrasion and
wear resistance.
Constructional data
Name Value Unit
Grammage 7090 kg/m2 DPL floor coverings do not contain substances that are listed in
Abrasion Class EN 13329 AC1-AC6 - the "Candidate List of Substances of Very High Concern for
Product Form panel - Authorisation" REACH.
Thickness of the element 8 mm
This product contains
Length of the surface layer 300 - 2500 mm
substances listed in the candidate list (date: 02.03.2021)
Width of the surface layer 70 - 400 mm exceeding 0.1
Length and width of squared elements 250 - 700 mm percentage by mass: NO.
Density 800 - 1200 kg/m3
Environment and health during use
Performance data of the product in accordance with the
declaration of Reference service life
performance with respect to its essential characteristics The estimated service life of a floor covering depends e.g. on
according to the type of floor covering and the area of application, the user
EN 13329. and the maintenance of the product. Comparisons of different
floor coverings are only allowed if these parameters are
Base materials/Ancillary materials considered in a consistent way. A minimum service life of 20
2 Environmental-Product Declaration - European Producers of Laminate Flooring e.V. - DPL laminate flooring
years can be assumed according to Bundesinstitut für Bau-, considerably longer. The use stage is declared in this EPD for a
Stadt- und one-year usage.
Raumforschung (BBSR), technical service life can be
LCA: Calculation rules
includes benefits from all net flows in the end-of-life stage that
Declared Unit leave the
The declared unit is 1m² laminate flooring (7.09 kg/m², product boundary system after having passed the end-of-waste
thickness 8 mm) state. It is
Declared unit assumed that post-consumer DPL floor covering waste reaches
the end-of-waste state and is
Name Value Unit
100% incinerated in a European biomass power plant. Loads
Declared unit 1 m2 from material
Mass in kg per declared unit 7.09 kg/m² incineration and resulted potential energy credits (electricity
and thermal energy) are declared within module D.
For IBU core EPDs (where clause 3.6 is part of the EPD): for
average EPDs, an estimate of the robustness of the LCA
Module D contains the loads and potential benefits beyond
values must be made, e.g. concerning variability of the
the system boundary. Biogenic CO incorporated in the
production process, geographical representativeness and the 2
influence of background data and preliminary products wood fraction of the DPL flooring is released in module C3.
compared to the environmental impacts caused by actual
Geographic Representativeness
production.
Land or region, in which the declared product system is
manufactured, used or handled at the end of the product´s
System boundary lifespan: Europe
Type of EPD: cradle to gate with options, modules C1–C4, and
module D (A1–A3 + C + D and additional modules A4, A5 and
Comparability
B2).
Basically, a comparison or an evaluation of EPD data is only
possible if all the data sets to be compared were created
according to EN 15804 and the building context, respectively
Modules A1-A3 include processes that provide materials and
the product-specific characteristics of performance, are taken
energy input for the
into account.
system, manufacturing and transport processes up to the
factory gate, as well
as waste processing.
Factors for different thicknesses
Module A4 includes the transport to the point of installation.
The LCA results
for the DPL floor covering declared in this EPD refer to a
Module A5 includes packaging waste processing during the
laminate
construction process. A waste treatment in a waste incineration
flooring with a thickness of 8 mm, which meets the
plant is assumed. Credits from energy substitution are declared
requirements
in module D.
of the use classes: 21-23, 31-34 according to EN 13329, EN
ISO
Module B2 includes the cleaning of the floor covering. Provision
10874. In order to enable the
of water, cleaning agent and electricity for the cleaning of the
user of the EPD to calculate the results for different thicknesses
floor covering is considered, incl. waste water treatment. The
and
LCA results in this EPD are declared for a one-year usage.
use
classes the factors in the following table can be used for the
Module C includes dismantling (C1) and transport to waste a
calculation. For
treatment site (C2). It is assumed that dismantling is manually
A1-A3, A4, A5, C2, C3 and D the LCA results of the declared
done without environmental burdens, The DPL floor coverings
product (thickness
reach the end-of-waste state after dismantling and transport to
9mm) have to
a waste treatment site from the building.
be multiplied with these factors.
Module D
3 Environmental-Product Declaration - European Producers of Laminate Flooring e.V. - DPL laminate flooring
LCA: Scenarios and additional technical information
Characteristic product properties
Information on describing the biogenic carbon content at
Information on biogenic carbon
factory gate
Name ValueUnit
The biogenic carbon content quantifies the amount of biogenic
carbon in a kg
Biogenic carbon content in product 3.25
construction product leaving the factory gate, and it shall be C
separately declared for the product and for any accompanying Biogenic carbon content in accompanying kg
0.09
packaging. packaging C
Note: 1 kg biogenic carbon is equivalent to 44/12 kg of CO2
4 Environmental-Product Declaration - European Producers of Laminate Flooring e.V. - DPL laminate flooring
The common cleaning method for laminate floor coverings is
The following technical information is a basis for the declared damp mopping. Loose dirt should be removed by means of a
modules or can be used for developing specific scenarios in the dry mop or a vacuum cleaner.
context of a building assessment. In case of higher
requirements on hygiene (e.g. hospitals, care homes) or
Transport to the construction site (A4)
strongly frequented areas
Name Value Unit
(shops) a need for a higher cleaning frequency is possible.
Litres of fuel (consumption per kg) 0.00159 l/100km
Transport distance 250 km Reuse, recovery and/or recycling potentials (D), relevant
Capacity utilisation (including empty runs) 85 % scenario information
100% of post-consumer waste (7.09kg) is incinerated in a
Gross density of products transported 800-1200 kg/m3
biomass power plant.
Installation in the building (A5)
Name ValueUnit
In case a reference service life according to applicable ISO
Output substances following waste treatment on- 0.231 kg standards is declared then the assumptions and in-use
site packaging waste conditions underlying the determined RSL shall be declared. In
The amount of addition, it shall be stated that the RSL applies for the reference
installation waste varies and is not declared in this EPD. For the conditions only.
calculation
of the environmental impact of 1m² laminate flooring including a The same holds for a service life declared by the manufacturer.
certain amount of Corresponding information related to in-use conditions needs
installation waste the values for the production stage (A1-A3), not be provided if a service life taken from the list on service life
delivery (A4) by BNB is declared.
and end of life (C, D) have to be multiplied with the amount of
waste (e.g. 3% End of Life (C1-C4)
installation waste, factor 1.03).
Name Value Unit
Collected separately waste type 7.09 kg
Maintenance (B2)
Name Value Unit
Maintenance cycle (cleaning 120
Number/RSL
frequency per year) times/year
Water consumption (per year) 0.0068 m3
Auxiliary (per year) 0.0507 kg
Electricity consumption (per year) 0.074 kWh
5 Environmental-Product Declaration - European Producers of Laminate Flooring e.V. - DPL laminate flooring
LCA: Results
The results for module B2 refer to a period of one year.
Note: The results declared for EP-freshwater are
declared in the unit “P eq.” according to the European Platform on Life
Cycle Assessment (http://eplca.jrc.ec.europa.eu/LCDN/developerEF.xhtml).
This web link is provided in EN 15804+A2, clause 6.3.8.2.
DESCRIPTION OF THE SYSTEM BOUNDARY (X = INCLUDED IN LCA; ND = MODULE OR INDICATOR NOT DECLARED; MNR =
MODULE NOT RELEVANT)
BENEFITS
AND LOADS
CONSTRUCTION
BEYOND
PRODUCT STAGE PROCESS USE STAGE END OF LIFE STAGE
THE SYSTEM
STAGE
BOUNDARIE
S
la ire ta m w a Ry lp p u s tro p s n a rT g n iru tc a fu n a M e h t m o rf tro p s n a rTe tis e h t o t e ta g y lb m e s s A e s U e c n a n e tn ia M ria p e R tn e m e c a lp e R tn e m h s ib ru fe R y g re n e la n o ita re p Oe s u re ta w la n o ita re p Oe s u n o itc u rts n o c -e Dn o itilo m e d tro p s n a rT g n is s e c o rp e ts a W la s o p s iD -e s u e R-y re v o c e R-g n ilc y c e Rla itn e to p
A1 A2 A3 A4 A5 B1 B2 B3 B4 B5 B6 B7 C1 C2 C3 C4 D
X X X X X MND X MNR MNR MNR MND MND X X X MND X
RESULTS OF THE LCA - ENVIRONMENTAL IMPACT according to EN 15804+A2: 1 m² DPL Floor Covering (8mm)
Parameter Unit A1-A3 A4 A5 B2 C1 C2 C3 D
GWP-total kg CO 2 eq -2.65E+00 4.37E-02 2.77E-01 1.7E-01 0 4.23E-02 1.19E+01 -6.67E+00
GWP-fossil kg CO 2 eq 5.93E+00 4.34E-02 3.63E-02 1.58E-01 0 4.21E-02 0 -6.66E+00
GWP-biogenic kg CO 2 eq -8.58E+00 0 2.41E-01 -3.32E-02 0 0 1.19E+01 0
GWP-luluc kg CO 2 eq 6.25E-03 3.51E-04 4.13E-06 4.53E-02 0 3.4E-04 0 -5.28E-03
ODP kg CFC11 eq 2.7E-12 5.21E-18 4.47E-17 8.19E-09 0 5.05E-18 0 -7.91E-14
AP mol H+ eq 1.7E-02 1.43E-04 5.26E-05 4.67E-04 0 1.39E-04 0 3.99E-03
EP-freshwater kg P eq 1.41E-05 1.32E-07 7.65E-09 6.01E-06 0 1.28E-07 0 -9.72E-06
EP-marine kg N eq 8.1E-03 6.48E-05 1.79E-05 1.26E-04 0 6.28E-05 0 9.2E-04
EP-terrestrial mol N eq 6.2E-02 7.25E-04 2.41E-04 1.29E-03 0 7.02E-04 0 1.11E-02
kg NMVOC
POCP 1.56E-02 1.27E-04 4.8E-05 4.61E-04 0 1.23E-04 0 4.02E-03
eq
ADPE kg Sb eq 9.32E-07 3.11E-09 6.99E-10 1.37E-07 0 3.01E-09 0 -1.2E-06
ADPF MJ 1.19E+02 5.77E-01 7.48E-02 3.41E+00 0 5.59E-01 0 -1.14E+02
m3 world eq
WDP 6.61E-01 3.88E-04 3.06E-02 5.51E-02 0 3.75E-04 0 -3.85E-01
deprived
GWP = Global warming potential; ODP = Depletion potential of the stratospheric ozone layer; AP = Acidification potential of land and water; EP =
Eutrophication potential; POCP = Formation potential of tropospheric ozone photochemical oxidants; ADPE = Abiotic depletion potential for non-fossil
resources; ADPF = Abiotic depletion potential for fossil resources; WDP = Water (user) deprivation potential)
RESULTS OF THE LCA - INDICATORS TO DESCRIBE RESOURCE USE according to EN 15804+A2: 1 m² DPL Floor Covering
(8mm)
Parameter Unit A1-A3 A4 A5 B2 C1 C2 C3 D
PERE MJ 3.1E+01 3.24E-02 3.06E+00 9.13E-01 0 3.14E-02 0 -2.81E+01
PERM MJ 1.08E+02 0 -3.05E+00 0 0 0 -1.05E+02 0
PERT MJ 1.39E+02 3.24E-02 1.4E-02 9.13E-01 0 3.14E-02 -1.05E+02 -2.81E+01
PENRE MJ 9.54E+01 5.78E-01 5.79E-01 3.41E+00 0 5.6E-01 0 -1.14E+02
PENRM MJ 2.32E+01 0 -5.04E-01 0 0 0 -2.27E+01 0
PENRT MJ 1.19E+02 5.78E-01 7.48E-02 3.41E+00 0 5.6E-01 -2.27E+01 -1.14E+02
SM kg 7.74E-03 0 0 0 0 0 0 0
RSF MJ 0 0 0 0 0 0 0 0
6 Environmental-Product Declaration - European Producers of Laminate Flooring e.V. - DPL laminate flooring
NRSF MJ 0 0 0 0 0 0 0 0
FW m3 3.2E-02 3.76E-05 7.21E-04 1.41E-03 0 3.64E-05 0 -2.33E-02
PERE = Use of renewable primary energy excluding renewable primary energy resources used as raw materials; PERM = Use of renewable primary
energy resources used as raw materials; PERT = Total use of renewable primary energy resources; PENRE = Use of non-renewable primary energy
excluding non-renewable primary energy resources used as raw materials; PENRM = Use of non-renewable primary energy resources used as raw
materials; PENRT = Total use of non-renewable primary energy resources; SM = Use of secondary material; RSF = Use of renewable secondary fuels;
NRSF = Use of non-renewable secondary fuels; FW = Use of net fresh water
RESULTS OF THE LCA – WASTE CATEGORIES AND OUTPUT FLOWS according to EN 15804+A2:
1 m² DPL Floor Covering (8mm)
Parameter Unit A1-A3 A4 A5 B2 C1 C2 C3 D
HWD kg 3.71E-07 2.69E-08 1.09E-10 5.52E-05 0 2.6E-08 0 -4.53E-08
NHWD kg 1.25E-01 8.84E-05 7.15E-03 8.06E-03 0 8.56E-05 0 5E-03
RWD kg 4.01E-03 7.15E-07 3.94E-06 1.04E-04 0 6.93E-07 0 -9.6E-03
CRU kg 0 0 0 0 0 0 0 0
MFR kg 0 0 0 0 0 0 0 0
MER kg 0 0 0 0 0 0 7.09E+00 0
EEE MJ 0 0 3.78E-01 0 0 0 0 0
EET MJ 0 0 6.82E-01 0 0 0 0 0
HWD = Hazardous waste disposed; NHWD = Non-hazardous waste disposed; RWD = Radioactive waste disposed; CRU = Components for re-use;
MFR = Materials for recycling; MER = Materials for energy recovery; EEE = Exported electrical energy; EET = Exported thermal energy
RESULTS OF THE LCA – additional impact categories according to EN 15804+A2-optional:
1 m² DPL Floor Covering (8mm)
Parameter Unit A1-A3 A4 A5 B2 C1 C2 C3 D
Disease
PM 1.88E-07 7.7E-10 3.16E-10 1.88E-08 0 7.45E-10 0 -2.49E-08
incidence
IR kBq U235 eq 6.18E-01 1.03E-04 6.02E-04 2.1E-02 0 1E-04 0 -1.58E+00
ETP-fw CTUe 3.5E+01 4.08E-01 3.73E-02 1.88E+00 0 3.95E-01 0 -2.74E+01
HTP-c CTUh 5.04E-08 8.55E-12 2.17E-12 1.79E-10 0 8.28E-12 0 -2.67E-10
HTP-nc CTUh 6.56E-08 4.99E-10 1.16E-10 6.85E-09 0 4.83E-10 0 3.2E-08
SQP SQP 6.82E+02 2.03E-01 2E-02 2.57E+00 0 1.96E-01 0 -2.02E+01
PM = Potential incidence of disease due to PM emissions; IR = Potential Human exposure efficiency relative to U235; ETP-fw = Potential comparative
Toxic Unit for ecosystems; HTP-c = Potential comparative Toxic Unit for humans (cancerogenic); HTP-nc = Potential comparative Toxic Unit for humans
(not cancerogenic); SQP = Potential soil quality index
Disclaimer 1 – for the indicator IRP
This impact category deals mainly
with the eventual impact of low dose ionizing radiation on human health
of the nuclear fuel cycle. It does not consider effects due to
possiblenuclear accidents, occupational exposure nor due to radioactive
waste disposal in underground facilities. Potential ionizing radiation
from the soil, from radon and from some construction materials is also
not measured by this indicator.
Disclaimer 2 – for the indicators ADPE,
ADPF, WDP, ETP-fw, HTP-c, HTP-nc, SQP
The results of this environmental
impact indicator shall be used with care as the uncertainties on these
results are high or as there is limited experienced with the indicator.
References
Standards
ISO 14025
EN 14041 DIN EN ISO
EN 14041:2004: Resilient, textile and laminate floor coverings - 14025:2011-10, Environmental labels and declarations — Type
Essential characteristics. III
environmental declarations — Principles and procedures.
EN 13329
EN 13329: 2009-01: Laminate floor coverings - Elements with a EN 15804
surface layer based EN 15804:2019+A2, Sustainability of
on aminoplastic thermosetting resins - Specifications, construction works — Environmental Product Declarations —
requirements and Core rules for
test methods. the product category of construction products.
EN ISO 10874 IBU
ISO 10874:2009: Resilient, textile and laminate floor
coverings - Classification. Institut Bauen und Umwelt e.V.:
7 Environmental-Product Declaration - European Producers of Laminate Flooring e.V. - DPL laminate flooring
General Instructions for the EPD Programme of Institut Bauen Echterdingen, 2020 (http://documentation.gabi-software.com/)
und Umwelt e.V. Version 2.0, Berlin: Institut Bauen und
Umwelt e.V., 2021.
www.ibu-epd.com PCR Part A
Part A: Calculation Rules for the Life Cycle As-sessment and
Further Requirementson the Project Re-portaccording to EN
References 15804+A2:2019, InstitutBauen und Umwelt e.V. (IBU),
https://ibu-epd.com/
PCR Part B
Institut Bauen und Umwelt e.V.: Requirements on
the EPD for floor coverings, Version 1.2, 14.02.2018
BBSR
Bundesinstitut für Bau-, Stadt- und Raumforschung (BBSR): REACH
Nutzungsdauer von Bauteilen für Lebenszyklusanalyse nach
Bewertungssystem Nachhaltiges Bauen (BNB), 2011
Regulation (EC) No 1907/2006 of the European Parliament
and of the Council on the Registration, Evaluation,
GaBi Software Authorisation and Restriction
GaBi 10.0 dataset documentation for the software-system (CUP of Chemicals
2020.2) and databases, Sphera Solutions GmBH, Leinfelden-
8 Environmental-Product Declaration - European Producers of Laminate Flooring e.V. - DPL laminate flooring
Publisher
Institut Bauen und Umwelt e.V. +49 (0)30 3087748- 0
Hegelplatz 1 info@ibu-epd.com
10117 Berlin www.ibu-epd.com
Germany
Programme holder
Institut Bauen und Umwelt e.V. +49 (0)30 3087748- 0
Hegelplatz 1 info@ibu-epd.com
10117 Berlin www.ibu-epd.com
Germany
Author of the Life Cycle Assessment
Sphera Solutions GmbH +49 711 341817-0
Hauptstraße 111- 113 info@sphera.com
70771 Leinfelden-Echterdingen www.sphera.com
Germany
Owner of the Declaration
European Producers of Laminate Flooring (EPLF®) +49 521 13 69 760
Mittelstraße 50 info@eplf.com
33602 Bielefeld www.eplf.com,
Germany www.mylaminate.eu
9 Environmental-Product Declaration - European Producers of Laminate Flooring e.V. - DPL laminate flooring
