ENVIRONMENTAL-PRODUCT DECLARATION
as per ISO 14025 and EN 15804+A2
Owner of the Declaration Kingspan Insulation B.V.
Publisher Institut Bauen und Umwelt e.V. (IBU)
Programme holder Institut Bauen und Umwelt e.V. (IBU)
Declaration number EPD-KIN-20230012-CBD2-EN
Issue date 07.02.2023
Valid to 06.02.2028
Therma™ TW55
Kingspan Insulation B.V.
www.ibu-epd.com | https://epd-online.com
General Information
Kingspan Insulation B.V. Therma™ TW55
Programme holder Owner of the declaration
IBU – Institut Bauen und Umwelt e.V. Kingspan Insulation B.V.
Hegelplatz 1 Lingewei 8
10117 Berlin 4004LL Tiel
Germany Netherlands
Declaration number Declared product / declared unit
EPD-KIN-20230012-CBD2-EN Therma™ TW55
1m2, 120mm thickness, R = 5,45 m2.K/W
D
This declaration is based on the product category rules: Scope:
Insulating materials made of foam plastics, 08.03.2023 The insulation material Therma™ TW55 is produced by Kingspan
(PCR checked and approved by the SVR) Insulation at the manufacturing facilities in Winterswijk (the Netherlands)
and Kankaanpää (Finland). This EPD is based on weighted averages
which have been determined on the basis of the single values originating
Issue date from the different Kingspan Insulation factories.
Therma™ TW55 is an insulation board with a rigid thermoset
07.02.2023
polyisocyanurate (PIR) fibre-free insulation core, faced on both sides with
a low emissivity composite foil. Therma™ TW55 Framing Board is used as
thermal insulation for timber framing systems.
Valid to
06.02.2028 In order to enable the user of the EPD to calculate the LCA results for
different thicknesses, the EPD contains the respective calculation rules.
The owner of the declaration shall be liable for the underlying information
and evidence; the IBU shall not be liable with respect to manufacturer
information, life cycle assessment data and evidences.
The EPD was created according to the specifications of EN 15804+A2. In
the following, the standard will be simplified as EN 15804 bezeichnet.
Verification
The standard EN 15804 serves as the core PCR
Independent verification of the declaration and data according to ISO
Dipl.-Ing Hans Peters
14025:2011
(chairman of Institut Bauen und Umwelt e.V.)
internally X externally
Dr. Alexander Röder Vito D'Incognito,
(Managing Director Institut Bauen und Umwelt e.V.) (Independent verifier)
1 Environmental-Product Declaration - Kingspan Insulation B.V. - Therma™ TW55
Product
Performance data of the product in accordance with the
Product description/Product definition declaration of performance with respect to its essential
Therma™ TW55 is an insulation board with a rigid thermoset characteristics according to EN 13165 - Thermal insulation
polyisocyanurate (PIR) fibre-free insulation core, faced on both products for buildings - Factory made rigid polyurethane foam
sides with a low emissivity composite foil. The product is (PU) products - Specification
available in variable thicknesses from 20 mm up to 200 mm. The declaration of performance of the product can be found at
This EPD is based on a thickness of 120 mm and R D-value of www.kingspan.com.
5,45 m²·K/W. For the placing on the market of the product in the
Base materials/Ancillary materials
European Union/European Free Trade Association (EU/EFTA)
(with the exception of Switzerland) Regulation (EU) No. The product contains approximately 3,3 kg/m2 polyurethane
305/2011 (CPR) applies. The product needs a declaration of rigid foam and 0,3 kg/m2 multi-layer aluminium facings.
performance taking into consideration EN 13165 - Thermal The main materials of the polyurethane foam are MDI (between
insulation products for buildings - Factory made polyurethane 57-62 %), polyol (between 27-32 %) and a blowing agent
foam (PU) products - Specification and the CE-marking. For the (between 5-6 %). Due to the closed-cell structure (conform EN
application and use the respective national provisions apply. 13165), the blowing agent remains in the foam. Water, flame
retardants and additives are added (between 4-8 %).
Application
Therma™ TW55 Framing Board is used as thermal insulation In the current REACH regulations, polyurethane foam
for timber framing systems. insulation products are considered “articles” and are
exempt from the requirements of Articles 57 and 59(1)
Technical Data
of REACH Regulation (EC) No 1907/2006. These
The technical specifications of the products within the scope of products are not classified as “hazardous products”
the EPD shall be listed, including the reference to the test according to any current legislation, and can hence be
methods/test standards for each specification. declared as follows:
- This article contains substances listed in the
For products with CE marking, the technical specifications must
candidate list (date: 31.08.2022) exceeding 0.1
be specified in accordance with information in the declaration of
percentage by mass: no.
performance. The properties relevant to the product should be
- This article contains other carcinogenic, mutagenic,
specified in the table below. If no information is given for
reprotoxic (CMR) substances in categories 1A or 1B
properties, an explanation must be given in the background
which are not on the candidate list, exceeding 0.1
report to the EPD as to why the property is not relevant to the
percentage by mass: no.
product.
- Biocide products were added to this construction
product or it has been treated with biocide products
Constructional data (this then concerns a treated product as defined by the
Name Value Unit (EU) Biocidal Products Regulation No. 528/2012
(BPR): no.
Thermal conductivity according to
0.022 W(m.K)
EN 13165 Environment and health during use
Reaction to fire according to EN
E
13165 Reference service life
Compressive strength according to CS(10\Y) 100/ The reference service life is not to be declared in this
EN 13165 120/150 EPD as it does not cover the use stage.
Thickness tolerance according to
T2-T3
EN 13165
LCA: Calculation rules
Kankaanpää (Finland). The environmental impacts have been
Declared Unit calculated per plant over the calendar year 2021. Based on the
The declared unit (1 m²) and conversion factors are one-year production volume of Therma™ TW55 per plant, the
listed in the table below. individual environmental impacts are weighted.
Declared unit
The EPD is studied for a common product thickness of 120
Name Value Unit
mm. Multiplication factors are included to calculate impacts for
Declared unit 1 m2 other product thicknesses within the range of 20 to 200 mm.
Gross density 30 kg/m3
Grammage 3.6 kg/m2 For IBU core EPDs (where clause 3.6 is part of the EPD): for
average EPDs, an estimate of the robustness of the LCA
Layer thickness 0.12 m
values must be made, e.g. concerning variability of the
This EPD is based on a weighted average of the annual production process, geographical representativeness and the
production volume of three factories producing the products influence of background data and preliminary products
Therma™ TW55. compared to the environmental impacts caused by actual
production.
The scope of this EPD is the thermal insulation products
Therma™ TW55 as produced by Kingspan Insulation at the
System boundary
manufacturing facilities in Winterswijk (the Netherlands) and
2 Environmental-Product Declaration - Kingspan Insulation B.V. - Therma™ TW55
The type of EPD according to EN 15804 is: from energy substitution are declared in module D.
cradle to gate with options, modules C1–C4, and
module D (A1–A3, C, D and additional modules: Geographic Representativeness
A4, A5). Land or region, in which the declared product system is
manufactured, used or handled at the end of the product´s
The product stage is a mandatory information module and it lifespan: Europe
covers:
· A1, raw material extraction and processing, processing of
Comparability
secondary material input (e.g. recycling processes),
Basically, a comparison or an evaluation of EPD data is only
· A2, transport to the manufacturer,
possible if all the data sets to be compared were created
· A3, manufacturing, including provision of all materials,
according to EN 15804 and the building context, respectively
products and energy, packaging processing and its transport,
the product-specific characteristics of performance, are taken
as well as waste processing up to the end-of-waste state or
into account.
disposal of final residues
during the product stage.
Background database
Background data from GaBi ts Version 10 is used with
The construction process stage includes:
GaBi data sets CUP2022.1.
· A4 transport to the building site;
· A5 installation in the building including provision of all
materials, products and energy, as well as waste processing up
to the end-of-waste state or disposal of final residues during the
Factors for different thicknesses
construction process stage.
The LCA results for the insulation material declared in this EPD
refer to a product with a thickness of 120 mm. To enable the
The end-of-life stage is a mandatory information module and it
user of the EPD to calculate the results for different thicknesses
covers:
the factors in the following table can be used for the calculation.
· C1 de-construction, demolition;
The LCA results in chapter 5 have to be multiplied by these
· C2 transport to waste processing;
factors.
· C3 waste processing for reuse, recovery and/or recycling;
· C4 disposal (not applicable for this EPD) including provision
The scaling factors are applicable for the complete
and all transport, provision of all materials, products and related
product, where the multi-layer aluminium facings are
energy and water use.
for all product thicknesses equal and the foam inputs
are scaling upwards and downwards with other product
Environmental burden of the incineration (R1 > 60 %) of the
thicknesses.
product
at the end-of-life stage are assigned to the product system
(C3); resulting potential credits for thermal and electrical energy
LCA: Scenarios and additional technical information
Characteristic product properties on wooden pallets.
Information on biogenic carbon Within Module A3 the following packaging of the final
product is included:
The total mass of biogenic carbon containing materials is less - Polyethylene cover and wrap: 0,044 kg/m²
than 5 % of the total mass of the product and accompanying - Expanded Polystyrene skid: 0,008 kg/m²
packaging. - Wooden pallet: 0,040 kg/m²
Technical information
Transport to the building site (A4)
The following technical information is a basis for the
Name Value Unit
declared modules or can be used for developing
specific scenarios in the context of a building Litres of fuel 0.0103 l/100km
assessment. Transport distance 100 km
Gross density of products transported 30 kg/m3
Manufacturing (A3)
A polyethylene packaging foil is used. The products Installation into the building (A5)
are transported either on expanded polystyrene (EPS) skids or
3 Environmental-Product Declaration - Kingspan Insulation B.V. - Therma™ TW55
Name ValueUnit End of life (C1-C4)
Output substances following waste treatment on The assumptions for C1 are: diesel driven excavator (100 kW;
0.092 kg
site 0.2 litre fuel per ton excavated material). The assumptions for
The recycling of the packaging is considered in A5. C2 are: Truck Euro 6, diesel driven, 26-28 t gross weight,
assumed distance 50 km
Name ValueUnit
In case a reference service life according to applicable ISO Collected as mixed construction waste 3.6 kg
standards is declared then the assumptions and in-use
Energy recovery 3.575 kg
conditions underlying the determined RSL shall be declared. In
Recycling (aluminium content of the multi-layer
addition, it shall be stated that the RSL applies for the reference 0.025 kg
aluminium facings)
conditions only.
Reuse, recovery and/or recycling potentials (D), relevant
The same holds for a service life declared by the manufacturer. scenario information
Corresponding information related to in-use conditions needs Waste incineration with energy recuperation is assumed as an
not be provided if a service life taken from the list on service life end-of-life scenario
by BNB is declared.
4 Environmental-Product Declaration - Kingspan Insulation B.V. - Therma™ TW55
LCA: Results
In Table 1 "Description of the system boundary", all declared modules shall be indicated with an "X"; all modules that are not declared
shall be indicated with "MND" (As default the modules B3, B4, B5 are marked as MNR – module not relevant). In the following tables,
columns can be deleted for modules that are not declared. Indicator values should be declared with three valid digits (eventually using
exponential form (e.g. 1,23E-5 = 0,0000123). A uniform format should be used for all values of one indicator.
If several modules are not declared and therefore have been deleted from the table, the abbreviations for the indicators can be
replaced by the complete names, while the readability and clear arrangement should be maintained; the legends can then be deleted.
If due to relevant data gaps, an indicator cannot be declared in a robust way, then the abbreviation “IND” (indicator not declared)
should be used for this indicator.
• 0 - calculated value is 0
• 0 - value falls under the cut-off
• 0 - assumption which exclude any flows (e.g. exported
electricity A1-A3)
• IND – in cases where the inventory does not support
the methodological approach or the calculation of the
specific indicator IND shall be used.
If no reference service life is declared (see chapter 2.13 "Reference Service Life"), the LCA results of the modules B1-B2 and B6-B7
shall refer to a period of one year. This shall then be indicated as an explanatory text below the tables. In addition, the formula for the
quantification of such B-modules over the total life cycle shall be provided.
DESCRIPTION OF THE SYSTEM BOUNDARY (X = INCLUDED IN LCA; ND = MODULE OR INDICATOR NOT DECLARED; MNR =
MODULE NOT RELEVANT)
BENEFITS
AND LOADS
CONSTRUCTION
BEYOND
PRODUCT STAGE PROCESS USE STAGE END OF LIFE STAGE
THE SYSTEM
STAGE
BOUNDARIE
S
la ire ta m w a Ry lp p u s tro p s n a rT g n iru tc a fu n a M e h t m o rf tro p s n a rTe tis e h t o t e ta g y lb m e s s A e s U e c n a n e tn ia M ria p e R tn e m e c a lp e R tn e m h s ib ru fe R y g re n e la n o ita re p Oe s u re ta w la n o ita re p Oe s u n o itc u rts n o c -e Dn o itilo m e d tro p s n a rT g n is s e c o rp e ts a W la s o p s iD -e s u e R-y re v o c e R-g n ilc y c e Rla itn e to p
A1 A2 A3 A4 A5 B1 B2 B3 B4 B5 B6 B7 C1 C2 C3 C4 D
X X X X X MND MND MNR MNR MNR MND MND X X X X X
RESULTS OF THE LCA - ENVIRONMENTAL IMPACT according to EN 15804+A2: 1m2 120mm Therma™ TW55
Parameter Unit A1-A3 A4 A5 C1 C2 C3 C4 D
GWP-total kg CO 2-Äq. 1.05E+01 3.03E-02 2.69E-01 2.31E-03 1.52E-02 7.79E+00 0 -3.23E+00
GWP-fossil kg CO 2-Äq. 1.07E+01 3.02E-02 2.68E-01 2.31E-03 1.51E-02 7.63E+00 0 -3.22E+00
GWP-biogenic kg CO 2-Äq. -2.34E-01 -4.17E-05 1.47E-05 3.09E-06 -2.09E-05 1.66E-01 0 -1.6E-02
GWP-luluc kg CO 2-Äq. 6.79E-03 1.68E-04 3.18E-06 2.85E-08 8.42E-05 1.43E-05 0 -3.67E-04
ODP kg CFC11-Äq. 2.73E-11 1.81E-15 4.78E-14 1.42E-16 9.04E-16 5.77E-13 0 -2.07E-11
AP mol H+-Äq. 2.23E-02 3.11E-05 3.35E-05 1.07E-05 1.56E-05 4.55E-03 0 -4.94E-03
EP-freshwater kg PO 4-Äq. 4.8E-05 9.01E-08 1.21E-08 4.65E-10 4.51E-08 1.56E-07 0 -4.25E-06
EP-marine kg N-Äq. 5.76E-03 1.02E-05 8.97E-06 5.1E-06 5.09E-06 2.2E-03 0 -1.19E-03
EP-terrestrial mol N-Äq. 5.95E-02 1.21E-04 1.52E-04 5.59E-05 6.06E-05 2.53E-02 0 -1.28E-02
kg NMVOC-
POCP 2.85E-02 2.74E-05 2.59E-05 1.45E-05 1.37E-05 5.64E-03 0 -3.38E-03
Äq.
ADPE kg Sb-Äq. 1.1E-05 2.52E-09 1.17E-09 9.44E-11 1.26E-09 1.58E-08 0 -4.71E-07
ADPF MJ 2.74E+02 4.03E-01 9.91E-02 3.12E-02 2.02E-01 2.02E+00 0 -5.39E+01
m3 world-Äq.
WDP 1.59E+00 2.71E-04 2.55E-02 4.29E-06 1.35E-04 7.72E-01 0 -3.53E-01
deprived
GWP = Global warming potential; ODP = Depletion potential of the stratospheric ozone layer; AP = Acidification potential of land and water; EP =
Eutrophication potential; POCP = Formation potential of tropospheric ozone photochemical oxidants; ADPE = Abiotic depletion potential for non-fossil
resources; ADPF = Abiotic depletion potential for fossil resources; WDP = Water (user) deprivation potential)
RESULTS OF THE LCA - INDICATORS TO DESCRIBE RESOURCE USE according to EN 15804+A2: 1m2 120mm Therma™
TW55
Parameter Unit A1-A3 A4 A5 C1 C2 C3 C4 D
PERE MJ 2.77E+01 2.29E-02 2.54E-02 1.18E-04 1.15E-02 3.54E-01 0 -1.53E+01
PERM MJ 0 0 0 0 0 0 0 0
PERT MJ 2.77E+01 2.29E-02 2.54E-02 1.18E-04 1.15E-02 3.54E-01 0 -1.53E+01
PENRE MJ 1.57E+02 4.04E-01 4.55E+00 3.13E-02 2.02E-01 1.15E+02 0 -5.39E+01
PENRM MJ 1.17E+02 0 -4.45E+00 0 0 -1.13E+02 0 0
5 Environmental-Product Declaration - Kingspan Insulation B.V. - Therma™ TW55
PENRT MJ 2.74E+02 4.04E-01 9.92E-02 3.13E-02 2.02E-01 2.02E+00 0 -5.39E+01
SM kg 0 0 0 0 0 0 0 0
RSF MJ 0 0 0 0 0 0 0 0
NRSF MJ 0 0 0 0 0 0 0 0
FW m3 7.35E-02 2.59E-05 6.05E-04 1.78E-07 1.3E-05 1.82E-02 0 -1.65E-02
PERE = Use of renewable primary energy excluding renewable primary energy resources used as raw materials; PERM = Use of renewable primary
energy resources used as raw materials; PERT = Total use of renewable primary energy resources; PENRE = Use of non-renewable primary energy
excluding non-renewable primary energy resources used as raw materials; PENRM = Use of non-renewable primary energy resources used as raw
materials; PENRT = Total use of non-renewable primary energy resources; SM = Use of secondary material; RSF = Use of renewable secondary fuels;
NRSF = Use of non-renewable secondary fuels; FW = Use of net fresh water
RESULTS OF THE LCA – WASTE CATEGORIES AND OUTPUT FLOWS according to EN 15804+A2:
1m2 120mm Therma™ TW55
Parameter Unit A1-A3 A4 A5 C1 C2 C3 C4 D
HWD kg 1.13E-07 1.94E-12 8.26E-12 1.03E-13 9.68E-13 2.76E-10 0 -6.67E-09
NHWD kg 2.84E-01 5.8E-05 2.41E-02 2.93E-06 2.9E-05 4.37E-02 0 -8.06E-02
RWD kg 3.21E-03 4.98E-07 4.12E-06 3.43E-08 2.49E-07 8.4E-05 0 -4.21E-03
CRU kg 0 0 0 0 0 0 0 0
MFR kg 0 0 0 0 0 2.54E-02 0 0
MER kg 0 0 1.07E-01 0 0 3.46E+00 0 0
EEE MJ 0 0 4.87E-01 0 0 1.32E+01 0 0
EET MJ 0 0 8.72E-01 0 0 2.36E+01 0 0
HWD = Hazardous waste disposed; NHWD = Non-hazardous waste disposed; RWD = Radioactive waste disposed; CRU = Components for re-use;
MFR = Materials for recycling; MER = Materials for energy recovery; EEE = Exported electrical energy; EET = Exported thermal energy
RESULTS OF THE LCA – additional impact categories according to EN 15804+A2-optional:
1m2 120mm Therma™ TW55
Parameter Unit A1-A3 A4 A5 C1 C2 C3 C4 D
Disease
PM 1.87E-07 1.8E-10 4.08E-10 1.21E-10 8.98E-11 1.27E-08 0 -4.3E-08
incidence
IR kBq U235-Äq. 3.79E-01 7.3E-05 5.66E-04 4.99E-06 3.65E-05 1.35E-02 0 -7.2E-01
ETP-fw CTUe 1.12E+02 2.8E-01 7.09E-02 2.17E-02 1.4E-01 6.96E-01 0 -1.22E+01
HTP-c CTUh 7.1E-09 5.65E-12 3.98E-12 4.02E-13 2.82E-12 5.21E-11 0 -6.33E-10
HTP-nc CTUh 6.03E-07 2.93E-10 4.03E-10 2.03E-11 1.47E-10 1.9E-09 0 -2.23E-08
SQP SQP 6.57E+01 1.39E-01 2.53E-02 8.61E-05 6.94E-02 4.26E-01 0 -9.29E+00
PM = Potential incidence of disease due to PM emissions; IR = Potential Human exposure efficiency relative to U235; ETP-fw = Potential comparative
Toxic Unit for ecosystems; HTP-c = Potential comparative Toxic Unit for humans (cancerogenic); HTP-nc = Potential comparative Toxic Unit for humans
(not cancerogenic); SQP = Potential soil quality index
Disclaimer 1 – for the indicator “Potential Human exposure efficiency relative to U235”.This impact category deals
mainly with the eventual impact of low-dose ionizing radiation on human health of the nuclear fuel cycle. It does
not consider effects due to possible nuclear accidents, occupational exposure or to radioactive waste disposal in
underground facilities. Potential ionizing radiation from the soil, radon and from some construction materials is
also not measured by this indicator.
Disclaimer 2 – for the indicators “abiotic depletion potential for non-fossil resources”, “abiotic depletion potential
for fossil resources”, “water (user) deprivation potential, deprivation-weighted water consumption”, “potential
comparative toxic unit for ecosystems”, “potential comparative toxic unit for humans – cancerogenic”, “Potential
comparative toxic unit for humans - not cancerogenic”, “potential soil quality index”. The results of this
environmental impact indicator shall be used with care as the uncertainties on these results are high as there is
limited experience with the indicator.
References
Biocidal Products Regulation No. 528/2012 (BPR)
Regulation (EU) No 528/2012 of the European EN 13165
Parliament and of the Council of 22 May 2012 EN 13165:2012+A2:2016: Thermal insulation products
concerning the making available on the market and for buildings. Factory made polyurethane foam (PU)
use of biocidal products products. Specification
CPR EN 15804
Regulation (EU) No. 305/2011 of the European EN 15804:2012+A2:2019+AC:2021, Sustainability of
Parliament and of the Council of 9 March 2011 laying construction works — Environmental Product
down harmonised condition for the marketing of Declarations — Core rules for the product category of
construction products and repealing Council Directive construction products.
89/106/EC
GaBi ts
ISO 14025 thinkstep AG: Leinfelden-Echterdingen GaBi Software-
EN ISO 14025:2011, Environmental labels and System and Database for Life Cycle Engineering 1992-
declarations — Type III environmental declarations — 2019
Principles and procedures.
6 Environmental-Product Declaration - Kingspan Insulation B.V. - Therma™ TW55
IBU 2021 Institut Bauen und Umwelt e.V., Berlin (pub.): Product
Institut Bauen und Umwelt e.V.: General Instructions Category Rules for Construction Products from the
for the EPD programme of Institut Bauen und Umwelt range of Environmental Product Declarations of Institut
e.V., Version 2.0, Berlin: Institut Bauen und Umwelt Bauen und Umwelt (IBU), Part B: Requirements on the
e.V., 2021. EPD for insulating materials made of foam
www.ibu-epd.com plastics. January 2019
LCA-tool REACH
Kingspan LCA tool, version 1.1. IBU-KSI-202001-LT1- Regulation (EC) No 1907/2006 of the European
EN. Parliament and of the Council on the Registration,
Developed by Sphera Solutions GmbH (formely Evaluation, Authorisation and Restriction of Chemicals
Thinkstep GmbH) (REACH)
https://echa.europa.eu/candidate-list-table;
PCR Version 1.7, Part A
Institut Bauen und Umwelt e.V., Berlin (pub.): Product Candidate list
Category Rules for Building-Related Products and https://echa.europa.eu/candidate-list-table; accessed
services, Part A: Calculation Rules for the Life Cycle 31.08.2022, 233 substances listed.
Assessment and Requirements on the Project Report The literature referred to in the Environmental Product
according to EN 15804+A2:2019 Declaration must be listed in full.Standards already fully quoted
November 2021 in the EPD do not need to be listed here again.
The current version of PCR Part A and PCR Part B of the PCR
PCR 2017, Part B document on which they are based must be referenced.
7 Environmental-Product Declaration - Kingspan Insulation B.V. - Therma™ TW55
Publisher
Institut Bauen und Umwelt e.V. +49 (0)30 3087748- 0
Hegelplatz 1 info@ibu-epd.com
10117 Berlin www.ibu-epd.com
Germany
Programme holder
Institut Bauen und Umwelt e.V. +49 (0)30 3087748- 0
Hegelplatz 1 info@ibu-epd.com
10117 Berlin www.ibu-epd.com
Germany
Author of the Life Cycle Assessment
Kingspan Insulation B.V. +31 (0) 543 543 210
Lingewei 8 info@kingspaninsulation.nl
4004LL Tiel www.kingspan.com
Netherlands
Owner of the Declaration
Kingspan Insulation B.V. +31 (0) 543 543 210
Lingewei 8 info@kingspaninsulation.nl
4004LL Tiel www.kingspan.com
Netherlands
8 Environmental-Product Declaration - Kingspan Insulation B.V. - Therma™ TW55
