ENVIRONMENTAL PRODUCT DECLARATION
as per ISO 14025 and EN 15804+A2
Owner of the Declaration dormakaba International Holding GmbH
Publisher Institut Bauen und Umwelt e.V. (IBU)
Programme holder Institut Bauen und Umwelt e.V. (IBU)
Declaration number EPD-DOR-20240261-CBA1-EN
Issue date 29.11.2024
Valid to 28.11.2029
Door Closer TS 79
dormakaba
www.ibu-epd.com | https://epd-online.com
General Information
dormakaba Door Closer TS 79
Programme holder Owner of the declaration
IBU – Institut Bauen und Umwelt e.V. dormakaba International Holding GmbH
Hegelplatz 1 DORMA Platz 1
10117 Berlin 58256 Ennepetal
Germany Germany
Declaration number Declared product / declared unit
EPD-DOR-20240261-CBA1-EN 1 piece of the product: Door closer TS 79 consisting of the following items:
• 1 door closer
• Product packaging
This declaration is based on the product category rules: Scope:
Building Hardware products, 01.08.2021 This Environmental Product Declaration refers to a specific door closer
(PCR checked and approved by the SVR) manufactured by dormakaba. The production site is located in Suzhou
(China).
Issue date The data represents the year 2022.
29.11.2024
The owner of the declaration shall be liable for the underlying information
and evidence; the IBU shall not be liable with respect to manufacturer
information, life cycle assessment data and evidences.
Valid to
28.11.2029 The EPD was created according to the specifications of EN 15804+A2. In
the following, the standard will be simplified as EN 15804.
Verification
The standard EN 15804 serves as the core PCR
Independent verification of the declaration and data according to ISO
14025:2011
internally X externally
Dipl.-Ing. Hans Peters
(Chairman of Institut Bauen und Umwelt e.V.)
Florian Pronold Matthias Klingler,
(Managing Director Institut Bauen und Umwelt e.V.) (Independent verifier)
1 Environmental Product Declaration - dormakaba - Door Closer TS 79
Product
Performance data of the product with respect to its
Product description/Product definition characteristics in accordance with the relevant technical
The dormakaba door closer TS 79 with its minimalistic closer provision which can be applied are mentioned above.
body size is ideally suited for use in office fitouts and apartment
entry doors. The ease and speed with which it can be installed, Base materials/Ancillary materials
the fact that its spring strength can be so easily adapted to the The major material composition including the packaging of the
door size by template position to suit various door sizes makes product is listed below:
it the ideal choice for application. Name Value Unit
Steel 58 %
For the use and application of the product the respective
Aluminium 30 %
national provisions at the place of use apply. For the door
closer TS 79 the standards which can be applied are the Packaging 7 %
following: Lubricants 4 %
• EN 1154 Zinc <1 %
• EN 1634-1 Plastics <1 %
• AS1905 Paper <1 %
The product includes partial articles which contain substances
The CE marking takes into account the proof of conformity with
listed in the Candidate List of REACH Regulation
the respective harmonized standards based on the legal
1907/2006/EC (date: 14.06.2023) exceeding 0.1 percentage by
provisions mentioned above. ...
mass: yes
Application
• Lead (Pb): 7439-92-1 (CAS-No.) is included in some of
The dormakaba TS 79 is ideally suited for use in office fitouts the alloys used. The concentration of lead in each
and apartment entry doors. individual alloy does not exceed 4% (by mass).
Technical Data
The Candidate List can be found on the ECHA website
The door closer TS 79 has following technical properties:
address: https:echa.europa.eu/de/home.
Name Value Unit Reference service life
Spring strength (adjustable by size by The reference service life of the door closer TS 79 amounts to
2/3/4 Size
power shoe and templating position) 20 years, depending on the application and frequency of use.
For repairs and renewals, suitable spare parts are available.
Standard doors ≤ 1100 mm
The door closer is tested and certified to EN 1154, meaning
Fire doors NA available
they are designed to withstand a minimum of 500,000 cycles.
Non-handed NA available
The reference service life amounts to 20 years. This
External doors, outward opening NA available corresponds with approx. 25,000 cycles per year.
Hold-open NA available
Arm type standard scissor arm NA available
Parallel arm bracket NA included
Backcheck NA available
Closing speed adjustable at 2 separate 180° – 15° /
degrees
valves 15° – 0°
Approved to AS1905 Part 1 Fire
Resistant Doors (Backcheck model NA available
only)
LCA: Calculation rules
Declared Unit Production - Module A1-A3
The product stage includes: — A1, raw material extraction,
The declared unit is 1 piece of the product: Door closer TS 79 processing and mechanical treatments, processing of
including packaging secondary material input (e.g. recycling processes), — A2,
Name Value Unit transport to the manufacturer, — A3, manufacturing and
assembly including provision of all materials, products and
Declared unit 1 piece/product
energy, as well as waste processing up to the end-of-waste
Mass of declared product without
1.6714 kg state.
packaging
Mass of packaging 0,1262 kg
Construction stage - Modules A4-A5
The construction process stage includes:
— A4, transport to the building site; — A5, installation into the
System boundary building; including provision of all materials, products and
The type of EPD is: cradle to gate with options, modules C1– energy, as well as waste processing up to the end-of-waste
C4, and module D (A1–A3 + C + D and additional modules: state or disposal of final residues during the construction
A4+ A5) process stage.
2 Environmental Product Declaration - dormakaba - Door Closer TS 79
Land or region, in which the declared product system is
End-of-life stage– Modules C1-C4 and D manufactured, used or handled at the end of the product´s
The end-of-life stage includes: — C1, de-construction, lifespan: Global
demolition: — C2, transport to waste processing; — C3, waste
processing for reuse, recovery and/or recycling; — C4,
disposal; including provision and all transport, provision of all Comparability
materials, products and related energy and water use. Module Basically, a comparison or an evaluation of EPD data is only
D (Benefits and loads beyond the system boundary) includes: possible if all the data sets to be compared were created
— D, recycling potentials, expressed as net impacts and according to EN 15804 and the building context, respectively
benefits. the product-specific characteristics of performance, are taken
into account. Background database: GaBi, SP40.
Geographic Representativeness
LCA: Scenarios and additional technical information
Name Value Unit
Characteristic product properties of biogenic carbon
Waste packaging (paper and plastic) 0.12 kg
Name ValueUnit
kg Reference service life
Biogenic carbon content in product -
C Name Value Unit
Biogenic carbon content in accompanying 0.05 kg Life Span according to the manufacturer 20 a
packaging C
End of life (C1-C4)
Note: 1 kg of biogenic carbon is equivalent to 44/12 kg of CO .
2
C1: The product dismantling from the building is done manually
without environmental burden.
C2: Transport to waste management is 50 km.
Suzhou (China) is considered for A3.
Name Value Unit
Collected separately waste type 1.6742 kg
Transport to the building site (A4)
Recycling 1.67 kg
Name Value Unit
Energy recovery 0.0042 kg
Litres of fuel 0.00276l/100km
Capacity utilisation (including empty runs) 55 % The product is disassembled in a recycling process. Material
recycling is then assumed for metals. The plastic components
Transport distance (ship) 10000 km
are assumed to be incinerated with energy recovery. The minor
Transport distance via truck (from habor to
500 km proportions of residues arising from the recycling process are
dormakaba logistic centre)
landfilled. Region for the End of Life is: Global.
Transport distance via truck (for scaling) 100 km
The product is transported via truck and ship. For Europe, the Reuse, recovery and/or recycling potentials (D), relevant
product is stored in the dormakaba logistic center in Germany. scenario information
The main distribution regions are Asia and the EU with the
Name Value Unit
calculated transport distances. In order to allow scaling to a
Recycling 100 %
specific point of installation 100 km is declared as well.
The collection rate is 100 %.
Installation into the building (A5)
3 Environmental Product Declaration - dormakaba - Door Closer TS 79
LCA: Results
DESCRIPTION OF THE SYSTEM BOUNDARY (X = INCLUDED IN LCA; MND = MODULE OR INDICATOR NOT DECLARED; MNR
= MODULE NOT RELEVANT)
Benefits and
Construction loads beyond
Product stage Use stage End of life stage
process stage the system
boundaries
la ire ta m w a Ry lp p u s tro p s n a rT g n iru tc a fu n a M e h t m o rf tro p s n a rTe tis e h t o t e ta g y lb m e s s A e s U e c n a n e tn ia M ria p e R tn e m e c a lp e R tn e m h s ib ru fe R y g re n e la n o ita re p Oe s u re ta w la n o ita re p Oe s u n o itc u rts n o c -e Dn o itilo m e d tro p s n a rT g n is s e c o rp e ts a W la s o p s iD -e s u e R-y re v o c e R-g n ilc y c e Rla itn e to p
A1 A2 A3 A4 A5 B1 B2 B3 B4 B5 B6 B7 C1 C2 C3 C4 D
X X X X X MND MND MNR MNR MNR MND MND X X X X X
RESULTS OF THE LCA - ENVIRONMENTAL IMPACT according to EN 15804+A2: 1 piece Door Closer TS 79
Parameter Unit A1-A3 A4 A5 C1 C2 C3 C4 D
GWP-total kg CO 2 eq 7.8E+01 1.37E-01 1.79E-01 0 7.28E-03 2.09E-01 0 -4.74E+00
GWP-fossil kg CO 2 eq 7.8E+01 1.34E-01 4.48E-03 0 6.95E-03 1.97E-01 0 -4.73E+00
GWP-biogenic kg CO 2 eq -1.71E-02 3.55E-03 1.74E-01 0 3.21E-04 1.26E-02 0 -1.3E-02
GWP-luluc kg CO 2 eq 6.24E-03 3E-06 2.94E-06 0 1.66E-07 1.12E-05 0 -5.52E-04
ODP kg CFC11 eq 2.94E-12 1.35E-17 3.22E-17 0 7.34E-19 1.01E-16 0 -2.74E-11
AP mol H+ eq 4.1E-01 2.24E-03 5.01E-05 0 6.96E-06 3.68E-05 0 -1.58E-02
EP-freshwater kg P eq 1.83E-05 2.93E-08 6.31E-09 0 1.49E-09 1.61E-08 0 -2.55E-06
EP-marine kg N eq 1.42E-01 5.96E-04 1.81E-05 0 2.21E-06 8.49E-06 0 -2.22E-03
EP-terrestrial mol N eq 1.56E+00 6.53E-03 2.26E-04 0 2.46E-05 1.68E-04 0 -2.37E-02
kg NMVOC
POCP 4.07E-01 1.67E-03 4.8E-05 0 6.26E-06 2.35E-05 0 -7.49E-03
eq
ADPE kg Sb eq 6.87E-05 3.76E-09 5.09E-10 0 2.09E-10 1.39E-09 0 -2.74E-05
ADPF MJ 9.96E+02 1.78E+00 5.65E-02 0 9.86E-02 9.39E-02 0 -6.1E+01
m3 world eq
WDP 2.95E+00 2.53E-04 2.22E-02 0 1.36E-05 2.14E-02 0 -2.55E-01
deprived
GWP = Global warming potential; ODP = Depletion potential of the stratospheric ozone layer; AP = Acidification potential of land and water; EP =
Eutrophication potential; POCP = Formation potential of tropospheric ozone photochemical oxidants; ADPE = Abiotic depletion potential for non-fossil
resources; ADPF = Abiotic depletion potential for fossil resources; WDP = Water (user) deprivation potential)
RESULTS OF THE LCA - INDICATORS TO DESCRIBE RESOURCE USE according to EN 15804+A2: 1 piece Door Closer TS 79
Parameter Unit A1-A3 A4 A5 C1 C2 C3 C4 D
PERE MJ 2E+01 5.69E-03 1.52E+00 0 3.11E-04 1.08E-01 0 -2.28E+01
PERM MJ 1.6E+00 0 -1.51E+00 0 0 -8.4E-02 0 0
PERT MJ 2.16E+01 5.69E-03 1.03E-02 0 3.11E-04 2.42E-02 0 -2.28E+01
PENRE MJ 9.96E+02 1.78E+00 5.65E-02 0 9.87E-02 1.31E-01 0 -6.11E+01
PENRM MJ 3.72E-02 0 0 0 0 -3.72E-02 0 0
PENRT MJ 9.96E+02 1.78E+00 5.65E-02 0 9.87E-02 9.4E-02 0 -6.11E+01
SM kg 3.23E-01 0 0 0 0 0 0 0
RSF MJ 0 0 0 0 0 0 0 0
NRSF MJ 0 0 0 0 0 0 0 0
FW m3 7.5E-02 1.03E-05 5.22E-04 0 5.58E-07 5.12E-04 0 -4.31E-02
PERE = Use of renewable primary energy excluding renewable primary energy resources used as raw materials; PERM = Use of renewable primary
energy resources used as raw materials; PERT = Total use of renewable primary energy resources; PENRE = Use of non-renewable primary energy
excluding non-renewable primary energy resources used as raw materials; PENRM = Use of non-renewable primary energy resources used as raw
materials; PENRT = Total use of non-renewable primary energy resources; SM = Use of secondary material; RSF = Use of renewable secondary fuels;
NRSF = Use of non-renewable secondary fuels; FW = Use of net fresh water
RESULTS OF THE LCA – WASTE CATEGORIES AND OUTPUT FLOWS according to EN 15804+A2:
1 piece Door Closer TS 79
Parameter Unit A1-A3 A4 A5 C1 C2 C3 C4 D
HWD kg 2.91E-07 1.73E-10 8.33E-11 0 9.57E-12 3.49E-10 0 -1.45E-06
NHWD kg 2.23E+00 1.82E-04 5.61E-03 0 1.01E-05 2.05E-02 0 -7.81E-01
RWD kg 2.14E-03 1.94E-06 2.97E-06 0 1.06E-07 3.54E-06 0 -5.65E-03
CRU kg 0 0 0 0 0 0 0 0
MFR kg 0 0 0 0 0 1.58E+00 0 0
MER kg 0 0 0 0 0 0 0 0
EEE MJ 0 0 2.71E-01 0 0 3.83E-01 0 0
EET MJ 0 0 4.91E-01 0 0 8.69E-01 0 0
4 Environmental Product Declaration - dormakaba - Door Closer TS 79
HWD = Hazardous waste disposed; NHWD = Non-hazardous waste disposed; RWD = Radioactive waste disposed; CRU = Components for re-use;
MFR = Materials for recycling; MER = Materials for energy recovery; EEE = Exported electrical energy; EET = Exported thermal energy
RESULTS OF THE LCA – additional impact categories according to EN 15804+A2-optional:
1 piece Door Closer TS 79
Parameter Unit A1-A3 A4 A5 C1 C2 C3 C4 D
Disease
PM 4.53E-06 3.74E-08 2.78E-10 0 3.66E-11 4.56E-10 0 -2.51E-07
incidence
IR kBq U235 eq 2.52E-01 2.78E-04 4.59E-04 0 1.51E-05 3.3E-04 0 -1.12E+00
ETP-fw CTUe 6.48E+02 1.26E+00 2.68E-02 0 6.99E-02 3.54E-02 0 -1.88E+01
HTP-c CTUh 1.65E-08 2.37E-11 1.42E-12 0 1.31E-12 3.04E-12 0 -4.6E-10
HTP-nc CTUh 6.67E-07 1.06E-09 6.14E-11 0 5.62E-11 3.03E-10 0 -3.19E-08
SQP SQP 3.58E+01 4.63E-03 1.5E-02 0 2.53E-04 2.81E-02 0 -1.38E+00
PM = Potential incidence of disease due to PM emissions; IR = Potential Human exposure efficiency relative to U235; ETP-fw = Potential comparative
Toxic Unit for ecosystems; HTP-c = Potential comparative Toxic Unit for humans (cancerogenic); HTP-nc = Potential comparative Toxic Unit for humans
(not cancerogenic); SQP = Potential soil quality index
Disclaimer 1 – for the indicator “Potential Human exposure efficiency relative to U235”. This impact category deals mainly with the
eventual impact of low-dose ionizing radiation on human health of the nuclear fuel cycle. It does not consider effects due to possible
nuclear accidents, occupational exposure or radioactive waste disposal in underground facilities. Potential ionizing radiation from the
soil, radon and from some construction materials is also not measured by this indicator.
Disclaimer 2 – for the indicators “abiotic depletion potential for non-fossil resources”, “abiotic depletion potential for fossil resources”,
“water (user) deprivation potential, deprivation-weighted water consumption”, “potential comparative toxic unit for ecosystems”,
“potential comparative toxic unit for humans – cancerogenic”, “Potential comparative toxic unit for humans - not cancerogenic”,
“potential soil quality index”. The results of this environmental impact indicator shall be used with care as the uncertainties on these
results are high as there is limited experience with the indicator.
This EPD was created using a software tool.
References
EN 1154 Further References
DIN EN 1154: 2003-04: Building hardware – Controlled
doorclosing devices – Requirements and test methods IBU 2021
(includes amendment A1:2002); German version EN1154:1996 General Instructions for the EPD programme of Institut Bauen
+ A1:2002 und Umwelt e.V. Version 2.0, Berlin: Institut Bauen und Umwelt
e.V., 2021. www.ibu-epd.com
EN 1634-1
EN 1634-1:2018-04; Fire resistance and smoke control tests GaBi ts software
fordoor and shutter assemblies, openable windows and Sphera Solutions GmbH
elements of building hardware - Part 1: Fire resistance test for Gabi Software System and Database for Life Cycle Engineering
door andshutter assemblies and openable windows 19922020
Version 10.0.0.71
AS 1905.1 University of Stuttgart
AS 1905.1:2015; Components for the protection of openings in Leinfelden-Echterdingen
fire-resistant walls Fire-resistant doorsets
GaBi ts documentation
EN 15804 GaBi life cycle inventory data documentation
EN 15804+A2:2019+AC:2021, (https://www.gabisoftware.com/support/gabi/gabidatabase-
Sustainability of construction works — Environmental Product 2020-lcidocumentation/).
Declarations — Core rules for the product category of
construction products LCA-tool dormakaba
Tool No.: IBU-DOR-202104-LT1-EN
ECHA Developed by Sphera Solutions GmbH
European Chemical Agency
PCR Part A
ISO 14025 PCR – Part A: Calculation Rules for the Life Cycle Assessment
DIN EN ISO 14025:201110, Environmental labels and and Requirements on the Project Re-port according to EN
declarations — Type III environmental declarations — 15804+A2:2019,
Principles and procedures Version 1.0, 2020, Institut Bauen und Umwelt e.V., www.ibu-
epd.com.
REACH
Regulation (EC) No 1907/2006 of the European Parliament and
of the Council on the Registration, Evaluation, Authorisation PCR Part B
and Restriction of Chemicals (REACH) PCR – Part B: Requirements on the EPD for Building Hardware
product, version 08/2021, Institut Bauen und Umwelt e.V.,
RoHS www.ibu-epd.com.
2011/65/EU, Directive on the restriction of the use of certain
hazardous substances in electrical and electronic equipment
5 Environmental Product Declaration - dormakaba - Door Closer TS 79
Publisher
Institut Bauen und Umwelt e.V. +49 (0)30 3087748- 0
Hegelplatz 1 info@ibu-epd.com
10117 Berlin www.ibu-epd.com
Germany
Programme holder
Institut Bauen und Umwelt e.V. +49 (0)30 3087748- 0
Hegelplatz 1 info@ibu-epd.com
10117 Berlin www.ibu-epd.com
Germany
Author of the Life Cycle Assessment
dormakaba International Holding GmbH +49 2333 793-0
DORMA Platz 1 info.de@dormakaba.com
58256 Ennepetal www.dormakaba.com
Germany
Owner of the Declaration
dormakaba International Holding GmbH +49 2333 793-0
DORMA Platz 1 info.de@dormakaba.com
58256 Ennepetal www.dormakaba.com
Germany
6 Environmental Product Declaration - dormakaba - Door Closer TS 79
