ENVIRONMENTAL PRODUCT DECLARATION
as per ISO 14025 and EN 15804+A2
Owner of the Declaration Hilti Austria Industrie GmbH
Publisher Institut Bauen und Umwelt e.V. (IBU)
Programme holder Institut Bauen und Umwelt e.V. (IBU)
Declaration number EPD-HIL-20240158-CBJ2-EN
Issue date 19.07.2024
Valid to 18.07.2029
MFT-FOX VTR
Hilti AG
www.ibu-epd.com | https://epd-online.com
General Information
Hilti AG MFT-FOX VTR
Programme holder Owner of the declaration
IBU – Institut Bauen und Umwelt e.V. Hilti Austria Industrie GmbH
Hegelplatz 1 Gewerbepark C 7
10117 Berlin 2821 Lanzenkirchen
Germany Austria
Declaration number Declared product / declared unit
EPD-HIL-20240158-CBJ2-EN The declared product is the MFT-FOX VTR 300 L 6,5 as a
representative product for the FOX VTR portfolio. The
declared unit is to kg of product. The
packaging is also included in the calculation.
This declaration is based on the product category rules: Scope:
Building metals, 01.08.2021 This document relates to the MFT-FOX VTR 300 L 6,5 as a representative
(PCR checked and approved by the SVR) product for the MFT-FOX VTR portfolio. FOX VTR products cover the
same applications and are equal in material constitution and have
therefore been summarized in this EPD.
Issue date The owner of the declaration shall be liable for the underlying information
and evidence; the IBU shall not be liable with respect to manufacturer
19.07.2024
information, life cycle assessment data and evidences.
The EPD was created according to the specifications of EN 15804+A2. In
Valid to
the following, the standard will be simplified as EN 15804.
18.07.2029
Verification
The standard EN 15804 serves as the core PCR
Independent verification of the declaration and data according to ISO
14025:2011
internally X externally
Dipl.-Ing. Hans Peters
(Chairman of Institut Bauen und Umwelt e.V.)
Florian Pronold Matthias Klingler,
(Managing Director Institut Bauen und Umwelt e.V.) (Independent verifier)
1 Environmental Product Declaration - Hilti AG - MFT-FOX VTR
Product
The application of the MFT FOX VTR product group is
Product description/Product definition explained on the basis of the Bracket MFT-FOX VTR 300 L 6,5.
MFT-FOX VTR is designed as a steel substructure bracket. The The bracket can be used for the fastening of substructures for
brackets are suitable for all façade cladding. The products are ventilated facades to concrete, masonry, SFS, and wood. The
used for fastening ventilated façade substructure to concrete, mounting of facade substructures on the main structure is
masonry, steel frame structure and wood. They enable supported by an auxiliary console that temporarily holds the
mounting façade substructures on the primary structure as a rails in position during fastening. The installation of vertical
helping hand bracket and can be used to install vertical support support rails is also possible. These fastening techniques are
rails. suitable for all facade claddings.
Product according to the CPR based on a hEN: Technical Data
For the placing on the market of the product in the European Technical documentation according to EN 1090-1.
Union/European Free Trade Association (EU/EFTA) (with the
Constructional data
exception of Switzerland) Regulation (EU) No. 305/2011 (CPR)
Name Value Unit
applies. The product needs a declaration of performance taking
into consideration EN [GS1] 1090-1:2009+A1:2011. Thickness Baseplate 2,5 mm
Length 60-300 mm
Length Steps 20 mm
Height 70 / 140 mm
Width 50 mm
Performance data of the product in accordance with
the declaration of performance with respect to its
essential characteristics according to EN 1090-
1:2009+A1:2011 Standard for execution of steel
structures and aluminium structures. The product is CE marked
accordingly. The structural parts made of stainless steel
correspond to following harmonized standards: EN 1090-1, DIN
EN 10088-1, DIN EN 1993-1-4 incl national annexes, DIN
18516-1.
Base materials/Ancillary materials
The raw material used for the production of this
product is steel alloy according to the
standard DIN EN 10088-1 with 910g (100% of product
weight). The alloy is a widely used extrusion alloy,
suitable for various applications.
This product ontains substances listed in the candidate list
(date 05.04.2022) exceeding 0.1 percentage by mass: no
This product contains other CMR substances in categories 1A
or 1B which
are not on the candidate list, exceeding 0.1 percentage by
mass: no
Biocide products were added to this construction
product or it has been treated with biocide products
(this then concerns a treated product as defined by the
(EU) Ordinance on Biocide Products No. 528/2012): no
Packaging
The packaging of this product is carton. This cardboard
packaging can be recycled.
Reference service life
The MFT-FOX VTR systems have a minimum service life
of 35 years when used as prescribed according to the
BBA Certificate (British Board of Agreement). However,
Application
the actual service life can be considerably longer.
LCA: Calculation rules
kg of steel substructure bracket, is also included in the
Declared Unit calculation at 0.03 kg.
The declared product here is a screw from HILTI AG with the
Declared unit and mass reference
designation MFT-FOX VTR 300 L as a representative product
from the MFT-VTR bracket portfolio. The declared unit refers to
1 kg of steel substructure bracket. The packaging, based on 1
2 Environmental Product Declaration - Hilti AG - MFT-FOX VTR
Name Value Unit They are transported by lorry and container ship. The following
flow charts illustrate the underlying production process.
Declared unit 1 kg
Gross density 8000 kg/m3
System boundary
Figure Information modules A 1 to A3 of the product.
Type of EPD: Cradle to factory gate with modules C1-C4 and D.
The following information modules are defined as
systemboundaries in this study:
Production stage (A1- A3):
- A1, raw material extraction,
- A2, transport to the manufacturer,
- A3, production. Figure Information modules A 1 to A3 of the packaging.
In the information modules C1 to C4, the deconstruction or
End of life (C1- C4): demolition from the building, the transport to waste disposal,the
- C1, dismantling/demolition, waste treatment and disposal of the product are
- C2, transport, recorded.Furthermore, reuse, recovery and recycling potentials
- C3, waste treatment , arereported in information module D.
- C4, disposal.
Geographic Representativeness
Land or region, in which the declared product system is
Reuse, recovery and recycling potential (D) manufactured, used or handled at the end of the product´s
lifespan: Europe
In order to accurately record the indicators and environmental
Comparability
impacts of the declared unit, a total of 8 information modules
Basically, a comparison or an evaluation of EPD data is only
are considered. The information modules A1 to A3 describe the
possible if all the data sets to be compared were created
provision of materials, transport to the production site and the
according to EN 15804 and the building context, respectively
production processes of the product itself.
the product-specific characteristics of performance, are taken
into account. The database referred to in this study is LCA for
Experts by Sphera. (V1 2023)
The primary products are sourced from the European Union.
LCA: Scenarios and additional technical information
The demolition of the bolt anchor from the building is calculated
Characteristic product properties of biogenic carbon in information module C1. The demolition is carried out using
The declared product does not contain any biogenic an electric chisel. The electrical energy consumption for the tool
Carbon. is assumed to be 0.5 MJ for the declared unit. The electricity
Note: 1 kg of biogenic carbon is equivalent to 44/12 kg of CO2. consumption is calculated using a European electricity mix.
Name Value Unit
Information on describing the biogenic carbon content at Collected as mixed construction waste 1 kg
factory gate
Recycling 0.85 kg
Name ValueUnit
Biogenic carbon content in accompanying kg Reuse, recovery and/or recycling potentials (D), relevant
packaging 0.01 C scenario information
Module D shows the substitution potential of primer steel using
Note: 1 kg of biogenic carbon is equivalent to 44/12 kg of CO .
2 a recycling scenario (85 % steel content of the product).
Name Value Unit
Stainless Steel 0,85 kg
End of life (C1 - C4)
3 Environmental Product Declaration - Hilti AG - MFT-FOX VTR
LCA: Results
DESCRIPTION OF THE SYSTEM BOUNDARY (X = INCLUDED IN LCA; MND = MODULE OR INDICATOR NOT DECLARED; MNR
= MODULE NOT RELEVANT)
Benefits and
Construction loads beyond
Product stage Use stage End of life stage
process stage the system
boundaries
la ire ta m w a Ry lp p u s tro p s n a rT g n iru tc a fu n a M e h t m o rf tro p s n a rTe tis e h t o t e ta g y lb m e s s A e s U e c n a n e tn ia M ria p e R tn e m e c a lp e R tn e m h s ib ru fe R y g re n e la n o ita re p Oe s u re ta w la n o ita re p Oe s u n o itc u rts n o c -e Dn o itilo m e d tro p s n a rT g n is s e c o rp e ts a W la s o p s iD -e s u e R-y re v o c e R-g n ilc y c e Rla itn e to p
A1 A2 A3 A4 A5 B1 B2 B3 B4 B5 B6 B7 C1 C2 C3 C4 D
X X X MND MND MND MND MNR MNR MNR MND MND X X X X X
RESULTS OF THE LCA - ENVIRONMENTAL IMPACT according to EN 15804+A2: 1 kg MFT-FOX VTR 300 L
Parameter Unit A1-A3 C1 C2 C3 C4 D
Global Warming Potential total (GWP-total) kg CO 2 eq 3.83E+00 5.86E-02 8.46E-03 2.58E-03 0 -2.84E+00
Global Warming Potential fossil fuels (GWP-fossil) kg CO 2 eq 3.82E+00 5.86E-02 8.38E-03 2.56E-03 0 -2.84E+00
Global Warming Potential biogenic (GWP-biogenic) kg CO 2 eq 3.32E-05 2.92E-05 0 0 0 0
Global Warming Potential luluc (GWP-luluc) kg CO 2 eq 3.62E-03 5.36E-06 7.64E-05 1.92E-05 0 -1.8E-03
Depletion potential of the stratospheric ozone layer (ODP) kg CFC11 eq 1.3E-11 5.76E-13 7.22E-16 4.28E-15 0 -9.91E-12
Acidification potential of land and water (AP) mol H+ eq 2.63E-02 8.92E-05 3.29E-05 1.34E-05 0 -2E-02
Eutrophication potential aquatic freshwater (EP-freshwater) kg P eq 4.96E-06 5.79E-08 3.01E-08 8.71E-09 0 -3.43E-06
Eutrophication potential aquatic marine (EP-marine) kg N eq 2.85E-03 2.52E-05 1.55E-05 6.13E-06 0 -1.99E-03
Eutrophication potential terrestrial (EP-terrestrial) mol N eq 3.17E-02 2.66E-04 1.73E-04 6.77E-05 0 -2.21E-02
Formation potential of tropospheric ozone photochemical oxidants kg NMVOC
8.73E-03 6.95E-05 2.98E-05 1.66E-05 0 -6.32E-03
(POCP) eq
Abiotic depletion potential for non fossil resources (ADPE) kg Sb eq 1.14E-04 2.84E-09 5.32E-10 2.74E-09 0 -8.94E-05
Abiotic depletion potential for fossil resources (ADPF) MJ 5.15E+01 1.29E+00 1.12E-01 5.04E-02 0 -3.81E+01
m3 world eq
Water use (WDP) 8.38E-01 4.92E-03 9.51E-05 4.98E-04 0 -6.54E-01
deprived
RESULTS OF THE LCA - INDICATORS TO DESCRIBE RESOURCE USE according to EN 15804+A2: 1 kg MFT-FOX VTR 300 L
Parameter Unit A1-A3 C1 C2 C3 C4 D
Renewable primary energy as energy carrier (PERE) MJ 1.1E+01 1.76E-01 7.94E-03 4.68E-03 0 -8.35E+00
Renewable primary energy resources as material utilization
MJ 4.5E-01 0 0 0 0 0
(PERM)
Total use of renewable primary energy resources (PERT) MJ 1.14E+01 1.76E-01 7.94E-03 4.68E-03 0 -8.35E+00
Non renewable primary energy as energy carrier (PENRE) MJ 5.15E+01 1.29E+00 1.12E-01 5.05E-02 0 -3.81E+01
Non renewable primary energy as material utilization (PENRM) MJ 0 0 0 0 0 0
Total use of non renewable primary energy resources (PENRT) MJ 5.15E+01 1.29E+00 1.12E-01 5.05E-02 0 -3.81E+01
Use of secondary material (SM) kg 0 0 0 0 0 0
Use of renewable secondary fuels (RSF) MJ 0 0 0 0 0 0
Use of non renewable secondary fuels (NRSF) MJ 0 0 0 0 0 0
Use of net fresh water (FW) m3 2.68E-02 2.95E-04 8.75E-06 1.44E-05 0 -2.07E-02
RESULTS OF THE LCA – WASTE CATEGORIES AND OUTPUT FLOWS according to EN 15804+A2:
1 kg MFT-FOX VTR 300 L
Parameter Unit A1-A3 C1 C2 C3 C4 D
Hazardous waste disposed (HWD) kg 8.1E-10 7.46E-11 4.16E-13 -1.31E-13 0 -6.03E-10
Non hazardous waste disposed (NHWD) kg 3.81E-01 2.84E-04 1.62E-05 1.33E-05 0 -2.98E-01
Radioactive waste disposed (RWD) kg 1.89E-03 2.01E-04 1.45E-07 6.77E-07 0 -1.36E-03
Components for re-use (CRU) kg 0 0 0 0 0 0
Materials for recycling (MFR) kg 0 0 0 0 0 0
Materials for energy recovery (MER) kg 0 0 0 0 0 0
Exported electrical energy (EEE) MJ 0 0 0 0 0 0
Exported thermal energy (EET) MJ 0 0 0 0 0 0
RESULTS OF THE LCA – additional impact categories according to EN 15804+A2-optional:
1 kg MFT-FOX VTR 300 L
Parameter Unit A1-A3 C1 C2 C3 C4 D
Disease
Incidence of disease due to PM emissions (PM) ND ND ND ND ND ND
incidence
Human exposure efficiency relative to U235 (IR) kBq U235 eq ND ND ND ND ND ND
Comparative toxic unit for ecosystems (ETP-fw) CTUe ND ND ND ND ND ND
Comparative toxic unit for humans (carcinogenic) (HTP-c) CTUh ND ND ND ND ND ND
Comparative toxic unit for humans (noncarcinogenic) (HTP-nc) CTUh ND ND ND ND ND ND
4 Environmental Product Declaration - Hilti AG - MFT-FOX VTR
Soil quality index (SQP) SQP ND ND ND ND ND ND
Disclaimer 1 – for the indicator “Potential Human exposure efficiency relative to U235”. This impact category deals mainly with the
eventual impact of low-dose ionizing radiation on human health of the nuclear fuel cycle. It does not consider effects due to possible
nuclear accidents, occupational exposure or radioactive waste disposal in underground facilities. Potential ionizing radiation from the
soil, radon and from some construction materials is also not measured by this indicator.
Disclaimer 2 – for the indicators “abiotic depletion potential for non-fossil resources”, “abiotic depletion potential for fossil resources”,
“water (user) deprivation potential, deprivation-weighted water consumption”, “potential comparative toxic unit for ecosystems”,
“potential comparative toxic unit for humans – cancerogenic”, “Potential comparative toxic unit for humans - not cancerogenic”,
“potential soil quality index”. The results of this environmental impact indicator shall be used with care as the uncertainties on these
results are high as there is limited experience with the indicator.
References
DIN EN 1090-2:2018-09 Regulation (EC) No 1907/2006
Standard for execution of steel structures and REACH RegulationRegulation (EU) No 528/2012on EU
aluminium structures Biocidal Products
DIN EN 1999-1-1 + DIN EN 1993-1-4 Other references
Eurocode 9: Design of steel structures and aluminum
structures - Part 1-4: BBA Certificate (British Board of Agreement)
General design rules The British Board of Agreement is a UK body issuing
certificates for construction products and systems and providing
DIN 18516-1 inspection services in support of their designers and installers.
Cladding for external walls, ventilated
Calculation rules: PCR - Part A
EN 1090-1:2009+A1:2011 Product category rules for construction products and services -
Standard for execution of steel structures and Calculation rules for the eco-balance and requirements for
aluminium structures thebackground report V1.3, Institut Bauen und Umwelt
DIN EN-10088-1 e.V.,08.2022.
Type of steel alloy
CML 2001 April. 2015Indicators for environmental impacts,
EN 15804 Leiden: UniversitätLeiden:
EN 15804:2012-04+A1 2013, Sustainability of http://cml.leiden.edu/software/datacmlia.html#downloads
construction works — Environmental Product (20.08.2022)
Declarations — Core rules for the product category of Product category rules for construction products – Part B
construction products Institut Bauen und Umwelt e.V, Berlin (pub.): Product
CategoryRules for Construction Products from the
ISO 14025 rangeofEnvironmental Product Declarations for Institut Bauen
DIN EN /ISO 14025:2011-10/, Environmental labels undUmwelt (IBU), PConstruction metals (01.08.2021)
and declarations — Type III environmental
declarations — Principles and procedures Sphera
LCA for Experts: Ganzheitliche Bilanzierung Leinfelden-
Regulation (EU) No. 305/2011 Echterdingen; Sphera Solution GmbH (Hrsg.)www.gabi-
Construction Product Regulation (CPR) software.com/deutsch/index/(19.02.2024)
5 Environmental Product Declaration - Hilti AG - MFT-FOX VTR
Publisher
Institut Bauen und Umwelt e.V. +49 (0)30 3087748- 0
Hegelplatz 1 info@ibu-epd.com
10117 Berlin www.ibu-epd.com
Germany
Programme holder
Institut Bauen und Umwelt e.V. +49 (0)30 3087748- 0
Hegelplatz 1 info@ibu-epd.com
10117 Berlin www.ibu-epd.com
Germany
Author of the Life Cycle Assessment
FIT-Umwelttechnik GmbH 05362 72 69 474
Westerstr. 13 bertram@fit-umwelttechnik.de
38442 Wolfsburg www.fit-umwelttechnik.com
Germany
Owner of the Declaration
Hilti Austria Industrie GmbH .
Gewerbepark C 7 juergen.hruby@hilti.com
2821 Lanzenkirchen www.hilti.group
Austria
6 Environmental Product Declaration - Hilti AG - MFT-FOX VTR
