ENVIRONMENTAL PRODUCT DECLARATION
as per ISO 14025 and EN 15804+A1
Owner of the Declaration Troldtekt A/S
Programme holder Institut Bauen und Umwelt e.V. (IBU)
Publisher Institut Bauen und Umwelt e.V. (IBU)
Declaration number EPD-TRO-20210192-IBA1-EN
Issue date 12.11.2021
Valid to 11.11.2026
Acoustic panels - unpainted
Troldtekt 35mm Natural Wood
www.ibu-epd.com | https://epd-online.com
Umwelt Produktdeklaration Name des Herstellers – Name des Produkts
1. General Information
Troldtekt A/S Natural Wood, unpainted
Programme holder Owner of the declaration
IBU – Institut Bauen und Umwelt e.V. Troldtekt A/S
Panoramastr. 1 Sletvej 2 A
10178 Berlin 8310 Tranbjerg
Germany Denmark
Declaration number Declared product / declared unit
EPD-TRO-20210192-IBA1-EN Acoustic panel "Natural Wood" - 1 m2, 35 mm
thickness - unpainted
This declaration is based on the product Scope:
category rules: This declaration represents the production, supply,
Wood cement - Mineral-bonded wooden composites, mounting, use, dismantling and disposal of 1 m2 (35
01.2019 mm thickness) of white cement-bonded wood wool
(PCR checked and approved by the SVR) acoustic panel "Natural Wood", produced by Troldtekt
A/S, with a reference service life of 50 years. The
production facility is located in Jutland, Denmark.
Issue date
Three scenarios represent its use in indoor conditions
12.11.2021
in Denmark, Sweden and Germany.
Valid to
The owner of the declaration shall be liable for the
11.11.2026
underlying information and evidence; the IBU shall not
be liable with respect to manufacturer information, life
cycle assessment data and evidences.
The EPD was created according to the specifications
of EN 15804+A1. In the following, the standard will be
simplified as EN 15804.
Verification
The standard EN 15804 serves as the core PCR
Independent verification of the declaration and data
according to ISO 14025:2010
Dipl. Ing. Hans Peters internally x externally
(chairman of Institut Bauen und Umwelt e.V.)
Dr. Alexander Röder Ms Jane Anderson
(Managing Director Institut Bauen und Umwelt e.V.)) (Independent verifier)
2. Product
2.1 Product description/Product definition 2.2 Application
Troldtekt Natural Wood acoustic panels are some of The panels are installed on the ceilings and walls in
the leading and preferred solutions for creating a good offices, businesses, schools, institutions, cultural sites,
indoor sound environment. They are sold in sports centers, swimming pools and private homes.
various thicknesses (20-35 mm) and dimensions
(width: 600 mm, lengths: 600/1200/2400 mm or width: 2.3 Technical Data
625 mm, lengths: 625/1250/2500 mm). The panels The table below indicates the technical specifications
can be unpainted or painted in a wide variety of of the panels in accordance with EN 13168, the
colors. standard for cement-bonded wood wool and double-
layer panels with cement-bonded wood wool, and EN
For the placing on the market of the product in the 13964, the standard for suspended ceilings.
European Union/European Free Trade Association
(EU/EFTA) (with the exception of Switzerland)
Regulation (EU) No. 305/2011 (CPR) applies. The
product needs a declaration of performance taking into
consideration EN 13964:2014, Suspended ceilings.
Requirements and test methods, and the CE-marking.
For the application and use, the respective national
provisions apply.
2 Environmental Product Declaration Troldtekt A/S – Troldtekt 35mm Natural Wood - unpainted
Technical specifications of the product covered in 2.9 Packaging
this EPD The product is packaged with plastic film and
Name Value Unit cardboard. The packaging material can be easily
Gross density 403 kg/m3 sorted and treated in dedicated waste recycling
Grammage 14,21 kg/m2 channels. The packaged product is delivered on a
Thermal conductivity acc. to DIN returnable wood pallet.
76 W/(mK)
52612
Water vapour diffusion resistance
- -
factor acc. to DIN 4108-4 2.10 Condition of use
Sound absorption coefficient (only Conditions of use are detailed
with reference to the - % here: https://www.troldtekt.com/Installation/Use_and_
corresponding component design) maintenance
Light reflection (measured by
DELTA Light and Optics 26,3 - 70,8 % 2.11 Environment and health during use
Reaction to fire B/S1/d0 Environmental and ecotoxicity risks from exposure to
Troldtekt panel products during use have been
assessed and found eligible to the following
certification schemes:
Performance data of the product in accordance with
the declaration of performance with respect to its  Finnish M1 classification
essential characteristics according to EN  Danish Indoor Climate
13168:2012+A1:2015, Thermal insulation products for  Blauer Engel
buildings. Factory made wood wool (WW) products.
 Cradle to Cradle
Specification, and EN 13964:2014, Suspended
ceilings. Requirements and test methods.
These certificates can be accessed
2.4 Delivery status here: https://www.troldtekt.com/Web-
The panel is usually distributed in length of 600, tools/Downloads/Certificates-and-tests
1200 or 2400 mm by 600 mm width or in length of 625,
1250 or 2500 mm by 625 mm width. It comes in 2.12 Reference service life
three thicknesses: 20, 25 and 35 mm. Additionally, The technical service life of the panel is superior to 50
several density ranges are available: Coarse, Fine, years. This EPD refers to the service lifetime indicated
Ultra-Fine and Extreme-Fine causing different by the BBSR table for the material 353.311 of type
densities (388-428 kg/m3). The panels are normally “Holzbekleidungen: Holz, Holzwerkstoff und
delivered in packs of 56 units on pallets. Mehrschichtleichtbauplatten”.
2.5 Base materials/Ancillary materials Because the panel is used in a building, in this EPD its
The composition of the finished product is a mix of reference service life is limited by the expected service
wood wool (32,7%), Portland cement (60,9%), water life of the building, which is commonly accepted as 50
(5,4%), as well as water glass (<1%) and accelerator years, at least as LCA timeframe.
(<1%). The composition is at dry basis at the factory
gate, as most of the water has evaporated during There is no influence of the ageing of the material on
drying, but water remains bound to the wood fibre and its technical performances.
cement paste (hydrated cement).
2.13 Extraordinary effects
2.6 Manufacture
Norway spruce logs from local forests (with a moisture Fire
content of about 65-70%) are received and the bark is Information on the fire performance according to EN
removed. The wood is stored for approximately six 13168.
months until the moisture content in the wood drops to
29%. The wood is then shredded to produce wool. The Fire protection
wood wool is mixed together with Portland cement, Name Value
water, and additives. The mixture is cast and cured Building material class B
using a heat press and dried with a biomass-fired Burning droplets d0
oven. The cast panel is milled to remove any material Smoke gas development S1
in excess and cut edges. After approximately 4 weeks
of curing, the panel can be painted before being stored Water
on a pallet and packaged to be transported to central No information on the product performance under the
distribution warehouses. unforseeable influence of water is available.
2.7 Environment and health during Mechanical destruction
manufacturing No information on the product performance under
Troldtekt is following its working environment closely. unforseeable mechanical destruction is available.
Both the physical working environment and sickness
absence are closely monitored. It is an ongoing 2.14 Re-use phase
process involving both leaders and factory workers. Currently, Troldtekt panels undergo thermal treatment
with energy recovery. Composting is also possible.
2.8 Product processing/Installation
Installation instructions are available here: Additional information on recycling
https://www.troldtekt.com/Installation options: https://www.troldtekt.com/~/media/Files/Info%
3 Environmental Product Declaration Troldtekt A/S – Troldtekt 35mm Natural Wood - unpainted
20sheets/English/Troldtekt_Recycling%20instructions
%20pdf.pdf Additional information on disposal
options: https://www.troldtekt.com/environment-and-
2.15 Disposal csr/product-life-cycle/recycling/
The product may be composted, thermally treated with
energy recovery, or landfilled. 2.16 Further information
For additional information on technical specifications,
European Waste Code: 10 13 11 (wastes from you may consult the Declaration Of
cement-based composite materials) Performance: https://www.troldtekt.com/Web-
tools/Downloads/DoPs 111121
Painted panels must be incinerated at end-of-life.
3. LCA: Calculation rules
3.1 Declared Unit is verified by a third party. Such representativeness is
The functional unit is 1 m2 of acoustic panel, in 35 mm also valid for the production of Portland cement, whose
thickness, corresponding to 14,21 kg of material with EPDs, however, were published in 2021 (white) and
unpainted finish, mounted on ceiling, with a reference 2017 (grey).
service life of 50 years.
Temporal, geographical and technological
Declared unit representativeness
Name Value Unit All data strictly related to the cement production is
Declared unit 1 m2 technologically, temporally, and geographically
Gross density 403 kg/m3 representative. The cement production data is less
Grammage 14.21 kg/m2 than 5 years old. However, since the improvement in
Layer thickness 0.035 m grey cement production processes in the meantime
have not been accounted for, the LCA results for the
Troldtekt panels based on grey cement can be said to
be conservative. The data used to model the
3.2 System boundary foreground inventory of acoustic panels dates from the
Cradle to grave production year of 2020. As for secondary data, some
most of the ecoinvent datasets are less than 3 years
3.3 Estimates and assumptions old.
Assumptions are described occasionally throughout
the section "LCA: Calculation rules". 3.7 Period under review
The primary data concerned with the manufacture (A1-
3.4 Cut-off criteria A3) relates to the production year 2020 and the data
The cut-off criterion is applied according to EN are based on the volumes produced on an annual
15804 Section 6.3.5 and PCR part A Section 5.6. basis.
All inputs and outputs for which data are available are
included in the LCA model. Data gaps are filled with 3.8 Allocation
conservative assumptions from average data (when Allocation of production data to the multiple produced
available) or with generic data and are documented types of panels (with the same functional unit) is
accordingly. performed based on the rules provided in EN 15804.
The following product flows have been omitted Sub-processes associated to painting have specially
according to the 1% cut-off rule: been allocated to the painted panels. Data such as
 Wooden pallet to transport the product waste generation and packaging have been allocated
to the entire production volume of panels in Troldtekt.
 Capital infrastructure (factory)
The only case of co-produced outputs is associated to
 Allocation of burden from wood logging to
wood logging. However, the environmental load is
residual wood fractions evenly distributed over all its co-products, such as
logs, energy wood, and bark.
3.9 Comparability
3.5 Background data
Basically, a comparison or an evaluation of EPD data
Two types of data source are used as secondary data:
is only possible if all the data sets to be compared
 Product-specific EPDs for the manufacture
were created according to EN 15804 and the building
and supply of Portland cement and water-
context, respectively the product-specific
based paint
characteristics of performance, are taken into account.
 Database ecoinvent v.3.6 cut-off
The used background database is ecoinvent v.3.6 cut-
off
3.6 Data quality
Statistical representativeness
The statistical representativeness of the product
system is very good. The input and output data
samples used to build inventories are based on the
entirety of the annual production of panels in 2020 and
4 Environmental Product Declaration Troldtekt A/S – Troldtekt 35mm Natural Wood - unpainted
4. LCA: Scenarios and additional technical information
Manufacture (A1-A3)
Data Installation into the building (A5)
Primary data is third-party verified and based on the Name Value Unit
production year 2020, within the facilities of Troldtekt Electricity consumption 0,060 kWh
A/S in Jutland (Denmark). Material loss (plastic film) 0,009 kg
Material loss (cardborad) 0,039 kg
End-of-waste state and use of by-products
For all processes supplying a residual material/waste Use phase (B1)
that originates the end-of-life phase of a product to the Prior to distribution and during the use phase (B1), the
product system to be used as input, the polluter-pay carbonation of the cement contained in the panel,
principle “100:0” is used. Some wooden by-products during use, is accounted for. Based on laboratory
generated during manufacture in Troldtekt end up as measurement, the panel will absorb up to 140 grams of
soil improvers externally (reaching end-of-waste state), carbon dioxide per kilogram of cement. Normalized to
and thus their biogenic carbon leaves Troldtekt's the reference flow, this corresponds to an uptake of
system boundary. approximately 0,9 kilograms of carbon dioxide by the
end of the service lifetime, including the uptake in A3.
Wind-certified electricity
All the electricity used to produce the panels in the Maintenance (B2)
Module A3 originates from Danish wind power, for As the panel does not require any maintenance except
which a certificate ensures the origin. It originates from for the occasional dusting, no maintenance module
a 1-3 MW offshore wind turbine, with transformation, (B2) is considered.
transmission and distribution losses and is modelled
correspondingly.
Name Value Unit
Carbon balance
Repair, replacement, refurbishment (B3, B4, B5)
Biogenic: Absorption of biogenic CO by the purchased
2 As the technical service life of the panel is superior to
wood has been considered in A1. Some of it is
the assumed service life of the building (50 years), no
released again during production in A3, some ends up
repair (B3), replacement (B4) or refurbishment (B5)
sequestered in soil, while the majority of the remaining
steps are considered.
biogenic CO , 8,86 kg, is retained in the finished
2
product and emitted during end-of-life incineration in
C4. Name Value Unit
Fossil: Absorption of some fossil CO , originating from
2
the calcination of limestone during cement production, Replacement (B4) / Refurbishment (B5)
happens when the cement is mixed with water in A3. A Name Value Unit
majority is absorbed during the use phase B1, and all
Information about reference service life is detailed in
the absorbed fossil CO is finally emitted during end-
2 2.12.
of-life incineration in C4.
Reference service life
Distribution to site (A4) and mounting (A5)
Name Value Unit
To consider the main geographical variants of the life
Reference service life (according to
cycle of Troldtekt Natural Wood panels, three 50 a
ISO 15686-1, -2, -7 and -8)
scenarios are developed, where the product is
Life Span (according to BBSR) 50 a
supplied, mounted, used and discarded in Aarhus
(Denmark), Hamburg (Germany) and Malmö Life Span according to the 75 a
(Sweden). An additional 50 km from the local manufacturer
warehouse to construction site is assumed.
Operational energy use (B6) and Operational water
use (B7)
Transport to the building site (A4) Name Value Unit
Name Value Unit Water consumption - m3
Litres of fuel 26,8 l/100km Electricity consumption - kWh
Transport distance to Denmark 160 km Other energy carriers - MJ
Transport distance to Germany 370 km Equipment output - kW
Transport distance to Sweden 394 km
Transport distance from End of life (C1-C4)
warehouse to local construction Name Value Unit
sites in 50 km Electricity use (for un-mounting) 0,060 kWh
Denmark/Germany/Sweden Transport (to material sorting
50 km
Capacity utilisation (including facility)
85 %
empty runs) Collected as mixed construction
14,21 kg
Gross density of products waste
403 kg/m3
transported Energy recovery 4,54 kg
Capacity utilisation volume factor 1 - Energy recovery efficiency 10 %
Energy recovered 9,26 MJ
5 Environmental Product Declaration Troldtekt A/S – Troldtekt 35mm Natural Wood - unpainted
The panel is un-mounted at the end of its reference
service life and driven to the regional waste
incineration plant. Energy is recovered from the wood
part of the panel at 10% efficiency.
Reuse, recovery and/or recycling potentials (D),
relevant scenario information
Name Value Unit
Electricity 2,20 MJ
Heat 7,07 MJ
The energy substituted from incineration of the panel's
wood component in C4 is considered being a split of
the Danish electricity grid mix (for electricity) and
natural gas (for heat).
Details on possible disposal routes
Aalborg Portland cement factory utilizes dust and
offcuts from the Troldtekt factory as a raw material in
new cement, i.e. in the technical circle. During
incineration in the cement kiln, the wood content in the
cement bonded wood wool panels replaces fossil fuels,
while the cement ends up as a raw material in new
cement, replacing virgin raw materials and heavy fossil
fuels, thereby avoiding a significant amount of CO
2
emissions. This scheme of wood wool waste as a raw
material can be scaled for construction site and
demolition waste. It will be gradually rolled out to all of
Denmark in the period 2021-2023. Once Denmark has
documented economic and environmental benefits to
be gained by including wood wool waste in the
production of new cement rather than going to waste
incineration or landfill, dialogue with municipalities and
local cement producers in the primary markets of
Troldtekt is initiated to facilitate similar schemes
regionally or nationally.
6 Environmental Product Declaration Troldtekt A/S – Troldtekt 35mm Natural Wood - unpainted
5. LCA: Results
Note: Global Warming Potential (GWP) indicator includes CO of both biogenic and fossil origin.
2
Also, GWP results for Troldtekt Natural Wood (unpainted) for other delivery scenarios in respectively Germany
and Sweden, are 2,73E-1 kg CO and 2,88E-1 kg CO .
2 2
DESCRIPTION OF THE SYSTEM BOUNDARY (X = INCLUDED IN LCA; MND = MODULE NOT DECLARED;
MNR = MODULE NOT RELEVANT)
BENEFITS AND
CONSTRUCTI LOADS
PRODUCT STAGE ON PROCESS USE STAGE END OF LIFE STAGE BEYOND THE
STAGE SYSTEM
BOUNDARIES
7 Environmental Product Declaration Troldtekt A/S – Troldtekt 35mm Natural Wood - unpainted
lairetam
waR
ylppus tropsnarT
gnirutcafunaM
eht
morf
tropsnarT
etis
eht
ot
etag
ylbmessA esU
ecnanetniaM
riapeR
tnemecalpeR tnemhsibrufeR
ygrene
lanoitarepO esu
retaw
lanoitarepO esu
noitcurtsnoc-eD
noitilomed tropsnarT
gnissecorp
etsaW
lasopsiD -esueR -yrevoceR -gnilcyceR laitnetop
A1 A2 A3 A4 A5 B1 B2 B3 B4 B5 B6 B7 C1 C2 C3 C4 D
X X X X X X MND MNR MNR MNR MND MND X X MND X X
RESULTS OF THE LCA - ENVIRONMENTAL IMPACT according to EN 15804+A1: 1 m2 Natural Wood, 35
mm, unpainted, delivered and used in Denmark
Parameter Unit A1-A3 A4 A5 B1 C1 C2 C4 D
GWP [kg CO2-Eq.] 1.58E+0 1.36E-1 1.03E-1 -9.31E-1 6.50E-4 1.17E-1 1.01E+1 -7.03E-1
ODP [kg CFC11-Eq.] 3.64E-7 2.49E-8 1.67E-9 0.00E+0 2.81E-10 2.14E-8 8.13E-9 -4.87E-8
AP [kg SO2-Eq.] 4.94E-2 2.76E-4 6.03E-5 0.00E+0 1.59E-6 2.38E-4 6.72E-4 -1.02E-3
EP [kg (PO4)3--Eq.] 1.17E-2 5.67E-5 1.12E-4 0.00E+0 8.86E-7 4.88E-5 2.92E-4 -5.90E-4
POCP [kg ethene-Eq.] 3.12E-3 1.82E-5 2.70E-6 0.00E+0 8.88E-8 1.56E-5 5.26E-5 -8.41E-5
ADPE [kg Sb-Eq.] 6.01E-5 3.72E-6 2.12E-7 0.00E+0 1.82E-8 3.20E-6 8.86E-7 -1.66E-6
ADPF [MJ] 8.90E+1 2.07E+0 3.72E-1 0.00E+0 4.20E-2 1.79E+0 8.12E-1 -1.02E+1
GWP = Global warming potential; ODP = Depletion potential of the stratospheric ozone layer; AP = Acidification potential of land and water; EP =
Caption Eutrophication potential; POCP = Formation potential of tropospheric ozone photochemical oxidants; ADPE = Abiotic depletion potential for non-
fossil resources; ADPF = Abiotic depletion potential for fossil resources
RESULTS OF THE LCA - INDICATORS TO DESCRIBE RESOURCE USE according to EN 15804+A1: 1 m2
Natural Wood, 35 mm, unpainted, delivered and used in Denmark
Parameter Unit A1-A3 A4 A5 B1 C1 C2 C4 D
PERE [MJ] 7.47E+1 2.93E-2 1.60E-1 0.00E+0 3.91E-2 2.52E-2 1.07E+1 -2.24E+0
PERM [MJ] 9.33E+1 0.00E+0 0.00E+0 0.00E+0 0.00E+0 0.00E+0 0.00E+0 0.00E+0
PERT [MJ] 1.68E+2 2.93E-2 1.60E-1 0.00E+0 3.91E-2 2.52E-2 1.07E+1 -2.24E+0
PENRE [MJ] 9.04E+1 2.07E+0 3.72E-1 0.00E+0 4.20E-2 1.79E+0 8.12E-1 -1.02E+1
PENRM [MJ] 2.29E-3 0.00E+0 0.00E+0 0.00E+0 0.00E+0 0.00E+0 0.00E+0 0.00E+0
PENRT [MJ] 9.04E+1 2.07E+0 3.72E-1 0.00E+0 4.20E-2 1.79E+0 8.12E-1 -1.02E+1
SM [kg] 1.27E-2 0.00E+0 0.00E+0 0.00E+0 0.00E+0 0.00E+0 0.00E+0 0.00E+0
RSF [MJ] 0.00E+0 0.00E+0 0.00E+0 0.00E+0 0.00E+0 0.00E+0 0.00E+0 0.00E+0
NRSF [MJ] 0.00E+0 0.00E+0 0.00E+0 0.00E+0 0.00E+0 0.00E+0 0.00E+0 0.00E+0
FW [m³] 2.85E-2 3.54E-4 1.35E-4 0.00E+0 1.19E-5 3.05E-4 3.57E-4 -8.12E-4
PERE = Use of renewable primary energy excluding renewable primary energy resources used as raw materials; PERM = Use of
renewable primary energy resources used as raw materials; PERT = Total use of renewable primary energy resources; PENRE = Use of
non-renewable primary energy excluding non-renewable primary energy resources used as raw materials; PENRM = Use of non-
Caption
renewable primary energy resources used as raw materials; PENRT = Total use of non-renewable primary energy resources; SM = Use
of secondary material; RSF = Use of renewable secondary fuels; NRSF = Use of non-renewable secondary fuels; FW = Use of net fresh
water
RESULTS OF THE LCA – WASTE CATEGORIES AND OUTPUT FLOWS according to EN 15804+A1:
1 m2 Natural Wood, 35 mm, unpainted, delivered and used in Denmark
Parameter Unit A1-A3 A4 A5 B1 C1 C2 C4 D
HWD [kg] 4.70E-1 2.11E-3 1.54E-3 0.00E+0 5.40E-5 1.81E-3 1.88E-3 -2.24E-2
NHWD [kg] 1.15E+1 1.45E-1 1.17E-1 0.00E+0 1.12E-3 1.24E-1 7.87E-2 -7.70E-1
RWD [kg] 1.35E-4 1.42E-5 2.56E-6 0.00E+0 5.78E-7 1.22E-5 6.32E-6 -1.06E-5
CRU [kg] 1.25E-4 0.00E+0 0.00E+0 0.00E+0 0.00E+0 0.00E+0 0.00E+0 0.00E+0
MFR [kg] 3.76E-5 0.00E+0 0.00E+0 0.00E+0 0.00E+0 0.00E+0 0.00E+0 0.00E+0
MER [kg] 5.93E-4 0.00E+0 0.00E+0 0.00E+0 0.00E+0 0.00E+0 0.00E+0 0.00E+0
EEE [MJ] 0.00E+0 0.00E+0 0.00E+0 0.00E+0 0.00E+0 0.00E+0 2.20E+0 0.00E+0
EET [MJ] 0.00E+0 0.00E+0 0.00E+0 0.00E+0 0.00E+0 0.00E+0 7.07E+0 0.00E+0
HWD = Hazardous waste disposed; NHWD = Non-hazardous waste disposed; RWD = Radioactive waste disposed; CRU = Components
Caption for re-use; MFR = Materials for recycling; MER = Materials for energy recovery; EEE = Exported electrical energy; EEE = Exported
thermal energy
6. LCA: Interpretation
The estimated impact results are only relative cement and wood in the foreground processes. Global
statements which do not indicate the end points of the Warming Potential net emissions share is much larger
impact categories, exceeding threshold values, safety in C4 than in A1-A3 (see why in chart (2)), while other
margins or risks. impact categories in module D in general are avoided
in the waste system owing to the incineration of end-of-
Two charts are presented: (1) with the standard life panels and substitution of natural gas and Danish
lifecycle impact categories displaying the share of electricity mix. C4 also slightly follows emissions of
impacts across all lifecycle stages, and (2) displaying compounds associated to other impact categories. A
the total carbon balance of the Troldtekt product's relatively inefficient transportation of end-of-life panels
lifecycle system. to waste incineration causes emissions in especially
Abiotic depletion of non-fossil resources, Depletion of
Impacts from the A1-A3 modules are dominant in the stratospheric ozone, and Photochemical ozone
life cycle of the Troldtekt Natural Wood panel products. formation.
This is primarily caused by the acquisition and use of
The embodied emissions associated to the raw A1-A3 and some fossil CO taken up in A1-A3 and B1
2
materials (primarily cement) are the main cause of is re-emitted in C4. CO emissions occurring in the
2-eq
impacts, especially in terms of net Global Warming remaining modules are negligible.
Potential, with 9,7 kg CO for cement followed by
2-eq
minor impacts from additives. In general, direct The amount of wood stored in the product refers to a
emissions from the Troldtekt production site are negative contribution to Global Warming Potential,
relatively small. Abiotic depletion of fossil resources reducing the share of Global Warming Potential in A1-
appears from the burden of producing cement using A3. This is due to the sequestration of biogenic carbon
fossil raw material such as limestone and to a large of wood during tree growth. The sequestered carbon
extent fossil fuels. In terms of carbon balance, biogenic does not contribute to global warming as long as it is
CO in A1-A3 offsets nearly all the fossil CO stored in the biomass.
2 2
emissions in A1-A3. All biogenic CO sequestered in
2
8 Environmental Product Declaration Troldtekt A/S – Troldtekt 35mm Natural Wood - unpainted
The clinker (cement) production is the most critical
Summary process of the Troldtekt product system, but
Within the cradle to grave, the following aspects have inaccuracies around the amount used will not
been identified as major contributors, mainly in the invalidate the present conclusions.
categories Global Warming Potential and Abiotic
depletion of fossil resources: Notably, by introducing cements with less carbon
footprint into production could lead to significant
 Emissions from the clinker production from reductions of especially the Global Warming Potential
material indicator.
 Emissions from the clinker production from
fuel
 Substituted emissions from end of life
incineration
7. Requisite evidence
Technological Institute under DANAK accreditation
7.1 Testing of substances used 392. Report no. MAIC-2019-1418. Reporting of
A detailed assessment of substances used was measured concentrations in toluene equivalents
conducted by a DAkkS-accredited laboratory, based according to EN 16516. This test is basis for the Finish
on a sample (prepared according to EN 15443), M1 Material certificate as well as the Danish Indoor
available in the Test Report 2018P216294, using Climate labeling certificate.
inductively coupled plasma mass spectrometry (EN
16171) and X-ray fluorescence (EN 15309), for the AgBB overview of results (28 days [µg/m³])
following: Name Value Unit
 Heavy metals (cadmium, mercury, etc.) TVOC (C6 - C16) 12 μg/m3
 and other elements Sum SVOC (C16 - C22) 0 - 5 μg/m3
VOC without NIK 0 - 5 μg/m3
Carcinogenic Substances 1 μg/m3
7.2 Leaching
No leaching measurement was conducted according
AgBB overview of results (3 days [µg/m³])
to EN 717-1.
Name Value Unit
TVOC (C6 - C16) - μg/m3
Sum SVOC (C16 - C22) - μg/m3
7.3 VOC emissions
R (dimensionless) - -
Testing for VOC emissions has been conducted in
VOC without NIK - μg/m3
accordance with EN ISO 16000-6. Analysis of the air
Carcinogenic Substances - μg/m3
sampled on Tenax was performed at the Danish
8. References
Standards guarded hot plate apparatus; conversion of the
measured values for building applications. 1 June 1984
AgBB
AgBB, Ausschuss zur gesundheitlichen Bewertung von
Bauprodukten (Committee for Health-related
Evaluation of Building Products) DIN EN ISO 14025
DIN EN ISO 14025:2011, Environmental labels and
BBSR declarations – Type III environmental
BBSR, Bundesinstitut für Bau-, Stadt- und declarations – Principles and procedures, German and
Raumforschung (Federal Institute for Research on English versions EN ISO 14025:2011
Building, Urban Affairs and Spatial Development).
BBSR table: EN 13168
https://www.nachhaltigesbauen.de/fileadmin/pdf/baust EN 13168:2012+A1:2015, Thermal insulation products
off_gebauededaten/BNB_Nutzungsdauern_von_Bautei for buildings. Factory made wood wool (WW) products.
len_2017-02-24.pdf Specification
DIN 4108-4 EN 13964
DIN 4108-4:2017-03, Thermal insulation and energy EN 13964:2014, Suspended ceilings. Requirements
economy in buildings - Part 4: Hygrothermal design and test methods
values
EN 15309
DIN 52612-2 EN 15309:2007, Characterization of waste and soil.
DIN 52612-2, Testing of thermal insulating materials; Determination of elemental composition by X-ray
determination of thermal conductivity by means of the fluorescence
9 Environmental Product Declaration Troldtekt A/S – Troldtekt 35mm Natural Wood - unpainted
EN 15443 air by active sampling on Tenax TA sorbent, thermal
EN 15443:2011, Solid recovered fuels. Methods for the desorption and gas chromatography using MS or MS-
preparation of the laboratory sample FID
EN 15804 Product Category Rule A
EN 15804:2012, EN 15804:2012+A1 2013, Product Category Rule A, IBU, 2021, Part A,
Sustainability of construction works – Environmental Calculation Rules for the Life Cycle Assessment and
Product Declarations – Core rules for the product Requirements on the Project Report. v.2.0.1. IBU,
category of construction products. 2021.
EN 16171 Product Category Rule B
EN 16171:2016, Sludge, treated biowaste and soil. Product Category Rule B, IBU, 2019, Part B,
Determination of elements using inductively coupled Requirements on the EPD for Wood cement - Mineral-
plasma mass spectrometry (ICP-MS) bonded wooden composites. v.1.7. IBU, 2019.
EN 16449
EN 16449:2014, EN 16449:2014, Wood and wood- Further References
based products - Calculation of the biogenic carbon
content of wood and conversion to carbon dioxide General Programme Instructions, IBU 2016
General Programme Instructions for the Preparation of
EN 16516 EPDs at the Institut Bauen und Umwelt e.V. Version 1.,
EN 16516:2017+A1:2020, Construction products: Berlin: Institut Bauen und Umwelt e.V., 2016.
Assessment of release of dangerous substances.
Determination of emissions into indoor air Software/database
OneClick LCA software, Pre-verified EPD tool,
EN 717-1 Bionova: https://www.oneclicklca.com/
EN 717-1:2004, Wood-based Panels – Determination
of Formaldehyde Release – Formaldehyde emission Database: Ecoinvent v.3.6. cut-off (2019)
by the chamber method
ISO 16000-6
ISO 16000-6:2011, Indoor air - Part 6: Determination of
volatile organic compounds in indoor and test chamber
10 Environmental Product Declaration Troldtekt A/S – Troldtekt 35mm Natural Wood - unpainted
Publisher
Institut Bauen und Umwelt e.V. Tel +49 (0)30 3087748- 0
Panoramastr. 1 Fax +49 (0)30 3087748- 29
10178 Berlin Mail info@ibu-epd.com
Germany Web www.ibu-epd.com
Programme holder
Institut Bauen und Umwelt e.V. Tel +49 (0)30 - 3087748- 0
Panoramastr 1 Fax +49 (0)30 – 3087748 - 29
10178 Berlin Mail info@ibu-epd.com
Germany Web www.ibu-epd.com
Author of the Life Cycle
Assessment Tel 98777223
Aalborg Portland Fax 80815733
Rørdalsvej 44 Mail
92200 Aalborg Ø stefan.e.danielsson@cementirhol
Denmark ding.it
Web www.aalborgportland.dk
Owner of the Declaration
Troldtekt A/S Tel +45 8747 8100
Sletvej 2A Fax +45 8747 8111
8310 Tranbjerg J Mail sales@troldtekt.dk
Denmark Web https://www.troldtekt.com
