ENVIRONMENTAL PRODUCT DECLARATION
as per ISO 14025 and EN 15804+A2
Owner of the Declaration DBC, EFCC, FEICA, IVK
Programme holder Institut Bauen und Umwelt e.V. (IBU)
Publisher Institut Bauen und Umwelt e.V. (IBU)
Declaration number EPD-FEI-20220106-IBG1-EN
Issue date 01.06.2022
Valid to 31.05.2027
Products based on polyurethane or silane-modified
polymer, group 2
DBC - Deutsche Bauchemie e.V.
EFCC - European Federation for Construction Chemicals
FEICA - Association of the European Adhesive and Sealant Industry
IVK - Industrieverband Klebstoffe e.V.
www.ibu-epd.com | https://epd-online.com
Umwelt Produktdeklaration Name des Herstellers – Name des Produkts
1. General Information
DBC - Deutsche Bauchemie e.V. Products based on polyurethane or
EFCC - European Federation for silane-modified polymer, group 2
Construction Chemicals
FEICA - Association of the European
Adhesive and Sealant Industry
IVK - Industrieverband Klebstoffe e.V.
Programme holder Owner of the declaration
IBU – Institut Bauen und Umwelt e.V. DBC, Mainzer Landstr. 55, D-60329 Frankfurt a.M.
Hegelplatz 1 EFCC, 172 Boulevard du Triomphe, B-1160 Brussels
10117 Berlin FEICA, Rue Belliard 40, B-1040 Brussels
Germany IVK, Völklingerstr. 4, D-40219 Düsseldorf
Declaration number Declared product / declared unit
EPD-FEI-20220106-IBG1-EN 1 kg product based on polyurethane or silane-
modified polymer; density 0.85 - 1.8 g/cm³
This declaration is based on the product Scope:
category rules: This verified EPD entitles the holder to bear the symbol
Reaction resin products, 07.2014 of the Institut Bauen und Umwelt e.V. It exclusively
(PCR checked and approved by the SVR) applies for products produced in Europe and for a
period of five years from the date of issue. This EPD
may be used by members of DBC, EFCC, FEICA and
Issue date
IVK and their members provided it has been proven
01.06.2022
that the respective product can be represented by this
EPD. For this purpose a guideline is available at the
Valid to secretariats of the four associations. The members of
31.05.2027 the associations are listed on the respective websites.
The owner of the declaration shall be liable for the
underlying information and evidence; the IBU shall not
be liable with respect to manufacturer information, life
cycle assessment data and evidences.
The EPD was created according to the specifications
of EN 15804+A2. In the following, the standard will be
simplified as EN 15804.
Verification
The standard EN 15804 serves as the core PCR
Independent verification of the declaration and data
according to ISO 14025:2011
Dipl. Ing. Hans Peters internally x externally
(chairman of Institut Bauen und Umwelt e.V.)
Dr. Alexander Röder Matthias Schulz
(Managing Director Institut Bauen und Umwelt e.V.)) (Independent verifier)
2. Product
2.1 Product description/Product definition fulfil manifold, often specific, functions in the
This EPD comprises reactive products based on construction, furnishing and repair of buildings. The
polyurethane (PU) or silane-modified polymer (SMP) product displaying the highest environmental impacts
with a volatile organic compound (VOC) content ≤1 % was used as a representative product for calculating
(VOC definition according to Decopaint Directive) and the Life Cycle Assessment results (worst-case
a castor oil/-derivatives content ≤10 %. The one- or approach).
two-component reactive PU products are
manufactured using polyols and isocyanates. Reactive For the placing on the market in the European
products based on SMP polymers are usually Union/European Free Trade Association (EU/EFTA)
manufactured as a one-component system from with the exception of Switzerland) products falling
polyols and alkoxysilane in a preliminary stage. The under Regulation (EU) No 305/2011 (CPR) need a
aqueous systems consist of (a) dispersion and are Declaration of Performance taking into consideration
crosslinked by a dispersible isocyanate. The products either the relevant harmonised European standard or
2 Environmental Product Declaration FEICA/EFCC/IVK/DBC – Products based on polyurethane or silane-modified polymer,
group 2
the European Technical Assessment and the CE self-expanding, ready to use polyurethane foam used
marking. For the application and use of the products for various construction applications. It consists of a
the respective national provisions apply. low viscous semi-fluid in a can that leaves the can as a
froth and immediately forms a polyurethane foam.
2.2 Application 12.1 Window & External Door Sealing & Insulation:
Products based on polyurethane or silane-modified Installing mechanically fixed external windows and
polymer, group 2, are used for the following doors with an OCF, as part of a system including
applications: sealants and tapes
12.2 Door Installation & Fixation:
Module 1: Adhesives for parquet and floor Fixing interior doors with an OCF
coverings 12.3 General Gap Filling:
Parquet adhesives in accordance with EN ISO 17178 Filling of regularly and irregularly shaped spaces
for wooden and parquet floors and flooring adhesives between at least two surfaces made of typical building
in accordance with EN ISO 22636 for floor coverings materials with a one-component foam (OCF)
Module 2: Reactive products for protecting and Module 13: Sealants for glazing
repairing concrete structures Two-component reactive sealants are to be used as
Products for increasing the durability of concrete and the second barrier of the structural hermetic seal in
reinforced concrete structures as well as for new insulating glass units.
concrete and for maintenance and repair work
(requirements 2.1), products for structural bonding of Module 14: Bonded glazing sealants
strengthening materials to an existing concrete One- and two-component reactive sealants are used
structure (requirements 2.2) and products for concrete for the bonding of insulating glass units in the window
injection for filling cracks, voids and interstices in frame.
concrete (requirements 2.3)
2.3 Technical Data
Module 3: Liquid-applied roof waterproofing kits The density of the products is between 0,85 and 1,8
Reactive products for waterproofing roof constructions g/cm³, other relevant technical data can be found in the
which are applied on site manufacturer’s technical documentation.
Module 4: Reactive products for liquid-applied Module 1: Reactive products as adhesive for
bridge deck waterproofing kits parquet and floor coverings
Products for liquid-applied waterproofing for use on The minimum requirements of EN ISO 17178 and EN
concrete bridge decks ISO 22636 must be maintained.
Module 5: Screed material, floor screeds and Module 2: Reactive products for protecting and
decorative floors repairing concrete structures
Products for screed/synthetic resin screed for use in 2.1 The requirements on essential characteristics for
floor constructions all intended uses in accordance with EN 1504-2,
Tables 1 and 5 must be maintained. These are:
Module 6: Reactive products as an adhesive for - Permeability to CO (EN 1062-6)
2
tiles - Water vapour permeability (EN ISO 7783-1/-2)
Tile adhesives for internal and external tile installations - Capillary absorption and permeability to water (EN
on walls, floors and ceilings 1062-3)
- Adhesive strength by pull-off test (EN 1542)
Module 7: Adhesives and sealants 2.2 Essential characteristics for all intended uses in
Reactive products for use as: accordance with EN 1504-4, Tables 3.1 and 3.2
· Structural and repair adhesives (manufacturer's declaration of performance)
· Surface and joint sealants 2.3 Requirements on essential characteristics for all
Applications in accordance with the manufacturer's intended uses in accordance with EN 1504-5, Table 3:
technical documentation/declaration of performance - Injectability (EN 1771)
- Viscosity (EN ISO 3219)
Module 8: Reactive products for watertight Further essential characteristics in accordance with the
covering kits manufacturer's technical documentation / declaration
Products for waterproofing floors and/or walls in wet of performance
rooms inside buildings
Module 3: Liquid-applied roof waterproofing kits
Module 9: Reactive products for liquid-applied The minimum requirements of EAD 030350-00-0402
waterproofing Liquid-applied roof waterproofing kits must be
Liquid applied products for waterproofing of buildings maintained. The essential characteristics are to be
specified in accordance with the European Technical
Module 10: Reactive products for waterproofing Assessment (ETA, specification no.).
and/or for pre-treating mineral substrates
Applications in accordance with the manufacturer's Module 4: Reactive products for liquid-applied
technical documentation bridge deck waterproofing kits
The minimum requirements of ETAG 033 Liquid-
Module 11: Liquid-applied waterproofing applied bridge deck waterproofing kits must be
membranes for use beneath ceramic tiling maintained. The essential characteristics are to be
specified in accordance with the European Technical
Module 12: One-component foam (OCF) Assessment (ETA, specification no.).
One component foam in a can is a one-component,
3 Environmental Product Declaration FEICA/EFCC/IVK/DBC – Products based on polyurethane or silane-modified polymer,
group 2
Module 5: Screed material, floor screeds and Module 11: Liquid-applied waterproofing
decorative floors membranes for use beneath ceramic tiling
The requirements on essential characteristics The minimum requirements on essential
according to EN 13813 'Screed material and floor characteristics according to EN 14891 - Liquid applied
screeds – Screed materials – Properties and water-impermeable products for use beneath ceramic
requirements'/ must be maintained. For synthetic resin tiling - Definitions, specifications and test methods-
screeds, these are: must be maintained. These are:
- Bond strength (EN 13892-8) - Initial tensile adhesion strength
- Reaction to fire (EN 13501-1) - Tensile adhesion strength after water contact
Further essential characteristics in accordance with the - Tensile adhesion strength after heat ageing
manufacturer's technical documentation/declaration of - Tensile adhesion strength after freeze-thaw cycles
performance - Waterproofing
- Crack bridging ability
Module 6: Reactive products as an adhesive for
tiles
Module 12: One-Component Foams
The requirements on essential characteristics
Physical data of the one-component foam must be
according to EN12004, must be maintained. These
indicated in accordance with the respective product
are:
standards; these can include, for example:
-Tensile adhesion strength after dry storage (EN
12004-2)
12.1 Window & External Door Sealing & Insulation
-Tensile adhesion strength after water immersion (EN
Tensile Strength EN 17333-4, Movement Capability
12004-2)
EN 17333-4, Curing Pressure EN 17333-2, Thermal
-Tensile adhesion strength after heat ageing (EN
conductivity EN 17333-5, Sound Insulation EN ISO
12004-2)
717-1, Post expansion EN 17333-2
-Tensile adhesion strength after freeze/thaw cycles
(EN 12004-2)
-Open time: Tensile strength (EN 12004-2) 12.2 Door Installation & Fixation
Further essential characteristics in accordance with the Shear Strength EN 17333-4, Tensile Strength
manufacturer's technical documentation EN 17333-4, Compression Strength EN 17333-4,
Curing pressure EN 17333-2
Module 7: Adhesives and sealants
Performance characteristics in accordance with the
12.3 General Gap Filling
manufacturer's technical documentation/declaration of
Sagging EN 17333-3 Other performance
performance
characteristics in accordance with the manufacturer's
technical documents / declaration of performance.
Module 8: Reactive products for watertight
covering kits
The minimum requirements of EAD 030352-00-0503 Module 13: Sealants for glazing
Liquid applied watertight covering kits for wet room Reactive sealants must comply with EN 1279-4
floors and/or walls must be maintained. The essential Performance characteristics in accordance with the
characteristics are to be specified in accordance with manufacturer's technical documentation/declaration of
the European Technical Assessment (ETA, performance
specification no.).
Module 14: Bonded glazing sealants
Module 9: Reactive products for liquid-applied Reactive sealants must comply with RAL-GZ 716 part
waterproofings 2 and ift-Guideline VE-08/4.
The minimum requirements of the test principles Performance characteristics in accordance with the
regarding the issuing of general building authority test manufacturer's technical documentation/declaration of
certificates for liquid-applied products for waterproofing performance
of buildings (PG-FLK) must be maintained. The
characteristics for the proof of usability are to be
specified in accordance with the test principles for
granting general building authority test certificates for
liquid applied polymer products for waterproofing
buildings
Module 10: Reactive products for waterproofing 2.4 Delivery status
and/or for pre-treating mineral substrates Liquid or pasty in containers made of tinplate or plastic
packed in separate or combi-containers for the
Name Value Unit required mixing ratio. Packages containing one kg of
Density acc. to EN ISO 2811-1 700 - 1800 kg/m3 product in different types of containers. Sealants in
Shore hardness A acc. to ISO 48- plastic cartridges and foil packs. Typical container
4 >15 sizes contain 10 to 25 kg of material. For major works,
Shore hardness D acc. to ISO 48- vats containing approx. 200 kg or IBCs (intermediate
4 >5 bulk containers) containing 1 tonne or more are also
used. The LCA is based on tinplate, plastic and wood
Viscosity acc. to ISO 3219-2 <100 Pas
packaging.
Other performance characteristics in accordance with
the manufacturer's technical
2.5 Base materials/Ancillary materials
documentation/declaration of performance
Products based on polyurethane or silane-modified
polymer with a VOC content ≤1 % and a castor oil/-
4 Environmental Product Declaration FEICA/EFCC/IVK/DBC – Products based on polyurethane or silane-modified polymer,
group 2
derivatives content ≤ 10% usually comprise a reactive type together with information on their hazardous
polymer and a crosslinking system. The polymer properties are listed in the safety data sheet of the
component contains polyether and/or polyester respective product.
polyols. Crosslinking takes place after installation on
site. In the case of two-component systems, this
involves the use of pre-polymers and polymers based 2.6 Manufacture
on typically methylene diphenyl diisocyanate (MDI), The components of the formulation are usually mixed
toluene diisocyanate (TDI), hexamethylene batch-wise and packaged for delivery.
diisocyanate (HDI) or isophorone diisocyanate (IPDI).
The resin mixing ratio is adjusted according to the 2.7 Environment and health during
stoichiometric requirements. Crosslinking starts directly manufacturing
after the components have been mixed. There are also As a general rule, no other environmental protection
one-component reactive polymer formulations based measures other than those specified by law are
on PU or SMP which crosslink in the presence of necessary.
moisture. They comprise prepolymers based on e.g.
MDI, TDI, HDI, IPDI or those with alkoxy-silane groups 2.8 Product processing/Installation
in the case of SMP formulations. In formulations with Products based on polyurethane or silane-modified
aqueous dispersions, dispersible isocyanates are used polymer, are processed by trowelling/knife-coating or
for crosslinking. The formulations can contain auxiliary rolling, pouring, spraying or injection.
materials such as accelerators, catalysts, wetting Precautions for safe handling and storage (e.g. air
agents, foam regulators and viscosity regulators for exchange, exhaust ventilation, personal protective
fine-tuning the product features. Typically, the products measures, precautions required in the handling of
covered by this EPD contain the following ranges of isocyanates, conditions for safe storage) must be
base materials and auxiliaries: observed in accordance with the information on the
Polyol component: up to approx. 50 % safety data sheet.
Crosslinking component: up to approx. 95 %
SMP component: up to approx. 80 % 2.9 Packaging
Plasticiser: ~ 0-25 % A detailed description of packaging is provided in
Additives / Pigments: ~ 0-30 % section 2.4. Empty containers and clean foils can be
Water: ~ 0-60 % recycled.
VOC: ≤1 % according to the Decopaint Directive
(mandatory)
Castor oil and derivatives: ≤10% (mandatory) 2.10 Condition of use
During the use phase, products based on polyurethane
These ranges are average values and the composition or silane-modified polymer are crosslinked and
of products complying with the EPD can deviate from essentially comprise an inert three-dimensional
these concentration levels in individual cases. More network. They are long-lasting products which protect
detailed information is available in the respective our buildings in the form of adhesives, coatings or
manufacturer's documentation (e.g. product data sealants as well as make an essential contribution in
sheets). retaining their function and long-term value.
Note: For companies to declare their products within
the scope of this EPD it is not sufficient to simply 2.11 Environment and health during use
comply with the product composition shown above. Option 1: Products for applications outside indoor
The application of this EPD is only possible for areas with permanent stays by people
member companies of DBC, EFCC, FEICA, and IVK During use, the reactive products lose their reactive
member associations and only for specific formulations properties and become inert. No risks are known for
with a total score below the declared maximum score water, air and soil if the products are used as
for a product group according to the associated designated.
guidance document. Option 2: Products for applications inside indoor
areas with permanent stays by people
When used in indoor areas with permanent stays by
1. substances from the “Candidate List of people, evidence of the emission performance of
Substances of Very High Concern for construction products in contact with indoor air must be
Authorisation” (SVHC) submitted according to national requirements (see
If this product contains substances listed in the chapter 7). No further influences by emissions on the
candidate list (latest version) exceeding 0.1 environment and health are known.
percentage by mass, the relevant information can be
found in the safety data sheet of the relevant product
covered by this model EPD. 2.12 Reference service life
2. CMR substances in categories 1A and 1B Cured products based on polyurethane or silane-
If this product contains other carcinogenic, mutagenic, modified polymer fulfil manifold, often specific functions
reprotoxic (CMR) substances in categories 1A or 1B in the construction or refurbishment of building
which are not on the candidate list, exceeding 0.1 structures. They decisively improve the usability of
percentage by mass, the relevant information can be building structures and significantly extend their
found in the safety data sheet of the relevant product original service lives. The anticipated reference service
covered by this model EPD. life depends on the specific installation situation and
3. Biocide products added to the construction the exposure associated with the product. It can be
product influenced by weathering as well as mechanical or
If this construction product contains biocide products, chemical loads.
the active substances, information on the
concentration and/or concentration range, the product
5 Environmental Product Declaration FEICA/EFCC/IVK/DBC – Products based on polyurethane or silane-modified polymer,
group 2
2.13 Extraordinary effects crosslinked products. If the crosslinked products can
be removed from construction products without large
Fire effort, thermal recovery is a practical recycling variant
Even without any special fire safety features, cured on account of their energy content. Minor adhesion is
products based on polyurethane or silane-modified not taken into consideration during disposal. It does
polymer comply with at least the requirements of EN not interfere with the disposal/recycling of the
13501-1 standard for fire classes E and Efl. In terms of remaining components/building materials.
the volumes applied, they have only a marginal
influence on the fire performance characteristics (e.g. 2.15 Disposal
smoke gas development) of the building structure in Residual material which cannot be used or recycled
which they have been installed. As crosslinked must be combined at a specified ratio and hardened.
polyurethane systems do not melt or drip, they do not Hardened product residue is not special waste. Non-
contribute towards spreading fire. hardened product residue is hazardous waste. Empty,
dried containers (free of drops and scraped clean) are
Water directed to the recycling process. Residue must be
Cured reactive products based on polyurethane or directed to proper waste disposal taking into
silane-modified polymer are chemically inert and consideration the local guidelines. The following waste
insoluble in water. They are often used to protect codes according to the European List of Waste
building structures from harmful water ingress or the (2000/532/EC) can apply:
effects of flooding. Hardened product residue:
European Waste Catalogue (EWC) code 080112
Mechanical destruction (waste paint and varnish with the exception of that
Mechanical destruction of cured reactive products mentioned in 08 01 11)
based on polyurethane or silane-modified polymer EWC code 080410 (waste adhesives and sealants
does not lead to any decomposition products which are other than mentioned in 08 04 09)
harmful to the environment or health.
2.16 Further information
2.14 Re-use phase More information is available on the manufacturer's
According to present knowledge, no environmentally product or safety data sheets and on the
harmful effects are generally anticipated in landfilling, manufacturer's websites or on request. Valuable
for example, as a result of de-construction and technical information is also available on the
recycling of building materials with adherent associations' websites.
3. LCA: Calculation rules
3.1 Declared Unit - A4 Transport to site
This EPD refers to the declared unit of 1 kg of product - A5 Installation, product applied into the building
based on polyurethane or silane-modified polymer, during A5 phase operations and packaging disposal.
group 2; applied into the building with a density of 0.85 This stage considers VOC emissions during the
- 1.8 g/cm³ in accordance with the IBU PCR part B for installation phase. The declared product does not
reaction resin products. contain substances in the formulation that directly emit
The results of the Life Cycle Assessment provided in (as) VOC, but VOCs are generated by a chemical
this declaration have been selected from the product reaction that are occurring during this phase. The end
with the highest environmental impact (worst-case of life for the packaging material considered is
scenario). described below:
Depending on the application, a corresponding -Incineration, for materials like plastic and wood.
conversion factor such as the density to convert -Landfill, for inert material like metals (where used).
volumetric use to mass must be taken into -C1-C2-C3-D
consideration. The building deconstruction (demolition process) takes
place in the C1 module which considers energy
The Declaration type is according to EN 15804: Cradle production and consumption in terms of diesel and all
to gate with options, modules C1–C3, and module D the emissions connected with the fuel-burning process
(A1–A3, C, D) and additional modules. to run the machines. After the demolition, the product
is transported to the end-of-life processing (C2
Declared unit module) where all the impacts related to the transport
Name Value Unit processes are considered. For precautionary principle
Declared unit 1 kg and as a worst-case scenario, thermal treatment is the
Gross density 0.85 - 1.8 g/cm³ only end-of-life scenario considered. This is modelled
Conversion factor to 1 kg - - by the incineration process (module C3) where the
product ends its life cycle.
Module D accounts for potential benefits that are
beyond the defined system boundaries. Credits are
3.2 System boundary generated during the incineration of wastes and related
Modules A1, A2 and A3 are taken into consideration in electricity produced that are occurring in the A5
the LCA: module.
- A1 Production of preliminary products
- A2 Transport to the plant 3.3 Estimates and assumptions
- A3 Production incl. provision of energy, production of For this EPD formulation and production data defined
packaging as well as auxiliaries and consumables and and collected by FEICA were considered. Production
waste treatment
6 Environmental Product Declaration FEICA/EFCC/IVK/DBC – Products based on polyurethane or silane-modified polymer,
group 2
waste was assumed to be disposed of by incineration LCA results. The background data sets used are less
without credits as a worst-case. than 4 years old.
An average of steel and plastic containers, and Production data and packaging are based on details
wooden pallets was considered in the LCA. provided by the manufacturer. The formulation used for
evaluation refers to a specific product.
3.4 Cut-off criteria The data quality of the background data is considered
All raw materials submitted for the formulations and to be good.
production data were taken into consideration.
The manufacture of machinery, plant and other 3.7 Period under review
infrastructure required for the production of the Representative formulations are valid for 2021.
products under review was not taken into consideration
in the LCA. 3.8 Allocation
Transport of packaging materials is excluded. Mass allocation has been applied when primary data
have been used and implemented into the LCA model.
3.5 Background data
Data from the GaBi database SP40 (2020) was used 3.9 Comparability
as background data. Basically, a comparison or an evaluation of EPD data
is only possible if all the data sets to be compared
3.6 Data quality were created according to EN 15804 and the building
Representative products were applied for this EPD and context, respectively the product-specific
the product in the group displaying the highest characteristics of performance, are taken into account.
environmental impact was selected for calculating the
The GaBi database SP40 (2020) was used.
4. LCA: Scenarios and additional technical information
Characteristic product properties Incineration 1 kg
Information on biogenic Carbon
The packaging material contains biogenic carbon
content which is presented below.
Information on describing the biogenic Carbon
Content at factory gate
Name Value Unit
Biogenic Carbon Content in product 0 kg C
Biogenic Carbon Content in
0.016 kg C
accompanying packaging
Transport to the building site (A4)
Name Value Unit
Transport distance 1000 km
Gross weight 34 - 40 t
Payload capacity 27 t
Assembly (A5)
Name Value Unit
Other resources for packaging
0.1 kg
material
Material loss 0.01 kg
Material loss regards the amount of product not used
during the application phase into the building. This
amount is 1% of the product, impacts related to the
production of this part are charged to the A5 module.
This percentage is considered as waste to disposal
and impacts of its end of life have been considered in
the LCA model and declared in A5.
End of life (C1-C3)
Name Value Unit
Collected as mixed construction
1 kg
waste
7 Environmental Product Declaration FEICA/EFCC/IVK/DBC – Products based on polyurethane or silane-modified polymer,
group 2
5. LCA: Results
DESCRIPTION OF THE SYSTEM BOUNDARY (X = INCLUDED IN LCA; ND = MODULE OR INDICATOR NOT
DECLARED; MNR = MODULE NOT RELEVANT)
BENEFITS AND
CONSTRUCTI LOADS
PRODUCT STAGE ON PROCESS USE STAGE END OF LIFE STAGE BEYOND THE
STAGE SYSTEM
BOUNDARIES
8 Environmental Product Declaration FEICA/EFCC/IVK/DBC – Products based on polyurethane or silane-modified polymer,
group 2
lairetam
waR
ylppus tropsnarT
gnirutcafunaM
eht
morf
tropsnarT
etis
eht
ot
etag
ylbmessA esU
ecnanetniaM
riapeR
tnemecalpeR tnemhsibrufeR
ygrene
lanoitarepO esu
retaw
lanoitarepO esu
noitcurtsnoc-eD
noitilomed tropsnarT
gnissecorp
etsaW
lasopsiD -esueR -yrevoceR -gnilcyceR laitnetop
A1 A2 A3 A4 A5 B1 B2 B3 B4 B5 B6 B7 C1 C2 C3 C4 D
X X X X X ND ND MNR MNR MNR ND ND X X X ND X
RESULTS OF THE LCA - ENVIRONMENTAL IMPACT according to EN 15804+A2: 1 kg of product based on
polyurethane or silane modified polymer, group 2
Core Indicator Unit A1-A3 A4 A5 C1 C2 C3 D
GWP-total [kg CO2-Eq.] 8.05E+0 5.27E-2 2.13E-1 2.79E-4 1.24E-2 2.21E+0 -9.50E-1
GWP-fossil [kg CO2-Eq.] 7.89E+0 5.22E-2 1.25E-1 2.66E-4 1.18E-2 2.21E+0 -9.47E-1
GWP-biogenic [kg CO2-Eq.] 1.50E-1 1.52E-4 8.81E-2 1.24E-5 5.42E-4 8.82E-5 -2.23E-3
GWP-luluc [kg CO2-Eq.] 2.17E-3 4.22E-4 2.51E-5 6.39E-9 2.79E-7 2.08E-5 -6.66E-4
ODP [kg CFC11-Eq.] 2.74E-9 6.27E-18 2.74E-11 2.84E-20 1.24E-18 2.62E-16 -9.93E-15
AP [mol H+-Eq.] 1.48E-2 1.56E-4 1.76E-4 3.60E-6 3.73E-5 1.31E-3 -1.33E-3
EP-freshwater [kg P-Eq.] 1.30E-5 1.59E-7 1.35E-7 5.75E-11 2.51E-9 4.40E-8 -1.23E-6
EP-marine [kg N-Eq.] 4.39E-3 6.96E-5 5.22E-5 1.63E-6 1.72E-5 6.31E-4 -3.43E-4
EP-terrestrial [mol N-Eq.] 4.60E-2 7.80E-4 5.77E-4 1.79E-5 1.89E-4 7.26E-3 -3.68E-3
POCP [kg NMVOC-Eq.] 1.49E-2 1.38E-4 7.25E-3 4.91E-6 3.39E-5 1.62E-3 -9.87E-4
ADPE [kg Sb-Eq.] 8.36E-6 3.74E-9 8.40E-8 8.06E-12 3.52E-10 4.65E-9 -1.56E-7
ADPF [MJ] 1.66E+2 6.94E-1 1.73E+0 3.81E-3 1.66E-1 5.87E-1 -1.61E+1
[m³ world-Eq
WDP 1.19E+0 4.66E-4 2.54E-2 5.27E-7 2.30E-5 2.17E-1 -9.86E-2
deprived]
GWP = Global warming potential; ODP = Depletion potential of the stratospheric ozone layer; AP = Acidification potential of land and water; EP =
Caption Eutrophication potential; POCP = Formation potential of tropospheric ozone photochemical oxidants; ADPE = Abiotic depletion potential for non-
fossil resources; ADPF = Abiotic depletion potential for fossil resources; WDP = Water (user) deprivation potential
RESULTS OF THE LCA - INDICATORS TO DESCRIBE RESOURCE USE according to EN 15804+A2: 1 kg of
product based on polyurethane or silane modified polymer, group 2
Indicator Unit A1-A3 A4 A5 C1 C2 C3 D
PERE [MJ] 9.46E+0 3.90E-2 6.93E-1 1.20E-5 5.25E-4 8.23E-2 -3.52E+0
PERM [MJ] 5.85E-1 0.00E+0 -5.85E-1 0.00E+0 0.00E+0 0.00E+0 0.00E+0
PERT [MJ] 1.01E+1 3.90E-2 1.08E-1 1.20E-5 5.25E-4 8.23E-2 -3.52E+0
PENRE [MJ] 1.42E+2 6.95E-1 2.25E+0 3.81E-3 1.67E-1 2.56E+1 -1.61E+1
PENRM [MJ] 2.55E+1 0.00E+0 -5.20E-1 0.00E+0 0.00E+0 -2.50E+1 0.00E+0
PENRT [MJ] 1.67E+2 6.95E-1 1.73E+0 3.81E-3 1.67E-1 5.87E-1 -1.61E+1
SM [kg] 0.00E+0 0.00E+0 0.00E+0 0.00E+0 0.00E+0 0.00E+0 0.00E+0
RSF [MJ] 0.00E+0 0.00E+0 0.00E+0 0.00E+0 0.00E+0 0.00E+0 0.00E+0
NRSF [MJ] 0.00E+0 0.00E+0 0.00E+0 0.00E+0 0.00E+0 0.00E+0 0.00E+0
FW [m³] 3.55E-2 4.52E-5 6.75E-4 2.16E-8 9.41E-7 5.11E-3 -4.08E-3
PERE = Use of renewable primary energy excluding renewable primary energy resources used as raw materials; PERM = Use of
renewable primary energy resources used as raw materials; PERT = Total use of renewable primary energy resources; PENRE = Use of
non-renewable primary energy excluding non-renewable primary energy resources used as raw materials; PENRM = Use of non-
Caption
renewable primary energy resources used as raw materials; PENRT = Total use of non-renewable primary energy resources; SM = Use
of secondary material; RSF = Use of renewable secondary fuels; NRSF = Use of non-renewable secondary fuels; FW = Use of net fresh
water
RESULTS OF THE LCA – WASTE CATEGORIES AND OUTPUT FLOWS according to EN 15804+A2:
1 kg of product based on polyurethane or silane modified polymer, group 2
Indicator Unit A1-A3 A4 A5 C1 C2 C3 D
HWD [kg] 4.35E-8 3.23E-8 6.08E-10 3.70E-13 1.62E-11 3.34E-10 -6.41E-9
NHWD [kg] 3.17E-1 1.06E-4 4.90E-2 3.90E-7 1.70E-5 1.11E-2 -7.44E-3
RWD [kg] 3.05E-3 8.60E-7 3.24E-5 4.09E-9 1.79E-7 2.37E-5 -1.20E-3
CRU [kg] 0.00E+0 0.00E+0 0.00E+0 0.00E+0 0.00E+0 0.00E+0 0.00E+0
MFR [kg] 0.00E+0 0.00E+0 0.00E+0 0.00E+0 0.00E+0 0.00E+0 0.00E+0
MER [kg] 0.00E+0 0.00E+0 0.00E+0 0.00E+0 0.00E+0 0.00E+0 0.00E+0
EEE [MJ] 0.00E+0 0.00E+0 2.12E-1 0.00E+0 0.00E+0 0.00E+0 0.00E+0
EET [MJ] 0.00E+0 0.00E+0 3.86E-1 0.00E+0 0.00E+0 0.00E+0 0.00E+0
HWD = Hazardous waste disposed; NHWD = Non-hazardous waste disposed; RWD = Radioactive waste disposed; CRU = Components
Caption for re-use; MFR = Materials for recycling; MER = Materials for energy recovery; EEE = Exported electrical energy; EEE = Exported
thermal energy
RESULTS OF THE LCA – additional impact categories according to EN 15804+A2-optional:
1 kg of product based on polyurethane or silane modified polymer, group 2
Indicator Unit A1-A3 A4 A5 C1 C2 C3 D
[Disease
PM ND ND ND ND ND ND ND
Incidence]
[kBq U235-
IRP ND ND ND ND ND ND ND
Eq.]
ETP-fw [CTUe] ND ND ND ND ND ND ND
HTP-c [CTUh] ND ND ND ND ND ND ND
HTP-nc [CTUh] ND ND ND ND ND ND ND
SQP [-] ND ND ND ND ND ND ND
PM = Potential incidence of disease due to PM emissions; IR = Potential Human exposure efficiency relative to U235; ETP-fw = Potential
Caption comparative Toxic Unit for ecosystems; HTP-c = Potential comparative Toxic Unit for humans (cancerogenic); HTP-nc = Potential
comparative Toxic Unit for humans (not cancerogenic); SQP = Potential soil quality index
Potential Human exposure efficiency relative to U235, Disclaimer 1 – This impact category deals mainly with the
eventual impact of low dose ionizing radiation on human health of the nuclear fuel cycle. It does not consider
effects due to possible nuclear accidents, occupational exposure or radioactive waste disposal in underground
facilities. Potential ionizing radiation from the soil, radon and (from) some construction materials is also not
measured by this indicator.
ADP minerals & metals, ADP fossil, WDP, ETF-fw, HTP-c, HTP-nc, SQP, Disclaimer 2 – The results of this
environmental impact indicator shall be used with care as the uncertainties on these results are high or as there is
limited experience with the indicator.
Additional environmental impact indicators (suggested by EN15804, table 4) are not declared in the EPD. The
results of this environmental impact indicator shall be used with care as the uncertainties on these results are high
and as there is limited experience with the indicator (see ILCD classification in EN 15804, table 5). For this
reason, results based on these indicators are not considered suitable for a decision-making process and are thus
not declared in the EPD.
6. LCA: Interpretation
The majority of impacts are associated with the (PERT) impacts comes from the consumption of
production phase (A1-A3). The most significant renewable energy resources required for the
contribution to the production phase impacts is the generation and supply of electricity. It should be noted
upstream production of raw materials as the main that Primary Energy Demand – Renewable (PERT)
driver. Another substantial contributor in the production generally represents a small percentage of the
phase, in the category of Abiotic depletion potential for production phase primary energy demand with the bulk
non-fossil resources (ADPminerals&metals), is the of the demand coming from non-renewable energy
steel sheet used as a packaging material. Emissions resources.
associated with the manufacturing of products also Transportation to the construction site (A4) and the
have some influence on the Formation potential of installation process (A5) make a low contribution to all
tropospheric ozone (POCP) in the production phase. In impacts.
all EPDs, CO is the most important contributor to The installation phase influences mainly the
2
Global Warming Potential (GWP). For the Acidification Photochemical ozone formation indicator, due to the
Potential (AP), NOx and SO contribute the largest emission of VOC during the operations. These
2
share. In some cases, HCl in water also impacts AP emissions are not directly related to the pre-products in
due to the use of TiO as a pigment. the resins, but they are related to the reaction products
2
The majority of life cycle energy consumption takes between pre-products and air components (water and
place during the production phase (A1-A3). Significant oxygen).
contributions to Primary Energy Demand – Non- The end-of-life phases influence climate change
renewable (PENRT) come from the energy resources indicators, due to the incineration processes occurring
used in the production of raw materials. The largest in the C3 module, the process used for modelling the
contributor to Primary Energy Demand – Renewable thermal treatment process of the resin.
7. Requisite evidence
VOC any of the existing regulations or in any of the existing
Special tests and evidence have not been carried out voluntary labelling programs for low-emitting products,
or provided within the framework of drawing up this as far as these
Model EPD. Some member states require special (1) include limits for the parameters TVOC, TSVOC,
documentation on VOC emissions into indoor air for carcinogens, formaldehyde, acetaldehyde, LCI limits
specific areas of application. This documentation, as for individual substances (including but not limited to
well as documentation for voluntary VOC labelling, has the European list of harmonized LCIs), and the R
to be provided separately and is specific for product in value;
question. (2) base their test methods on EN 16516;
(3) perform testing and apply the limits after 28 days
Evidence pertaining to VOC emissions shall show of storage in a ventilated test chamber, under the
- either an attestation of compliance with, conditions specified in EN 16516; some regulations
- or documentation of test data that are required in
9 Environmental Product Declaration FEICA/EFCC/IVK/DBC – Products based on polyurethane or silane-modified polymer,
group 2
and programs also have limits after 3 days, on top of - TSVOC: 100 µg/m³
the 28 days limits; - Each carcinogen: 1 µg/m³
(4) express the test results as air concentrations in - Formaldehyde: 100 µg/m³
the European Reference Room, as specified in EN - LCI: different per substance involved
16516. - R value: 1 (meaning that, in total, 100 % of the
combined LCI values must not be exceeded).
Examples of such regulations are the Belgian Royal Informative Annexes (2 tables):
Decree C-2014/24239, or the German AgBB/ ABG. Table 1 shown below is an overview of the most
Examples of such voluntary labelling programs are relevant regulations and specifications as of October
EMICODE, Blue Angel or Indoor Air Comfort. 2021, as regards requirements after 3 days of storage
in a ventilated test chamber.
Relevant test results shall be produced either by an Table 2 provides an overview of the most relevant
ISO 17025 accredited commercial test lab or by a regulations and specifications as of October 2021, as
qualified internal test lab of the manufacturer. regards requirements after 28 days of storage in a
Examples for the applied limits after 28 days of storage ventilated test chamber. Some details may be missing
in a ventilated test chamber are: in the table due to lack of space. Values given
- TVOC: 1000 µg/m³ represent maximum values/limits.
8. References
ETAG 033
Liquid applied bridge deck waterproofing kits ISO 48-4
10 Environmental Product Declaration FEICA/EFCC/IVK/DBC – Products based on polyurethane or silane-modified polymer,
group 2
ISO 48-4:2018, Rubber, vulcanized or thermoplastic - EN ISO 7783:2019-02, Paints and varnishes -
Determination of hardness- Part 4: Indentation Determination of water-vapour transmission properties
hardness by durometer method (Shore hardness) - Cup method
EN ISO 717-1 EN 12004
EN ISO 717-1:2020 Acoustics - Rating of sound EN12004:2012, Adhesives for ceramic tiles
insulation in buildings and of building elements -
Part 1: Airborne sound insulation EN 12004-1
EN 12004-1:2017, Adhesives for ceramic tiles – Part 1:
EN 1062-3 Requirements, assessment and verification of
EN 1062-3:2008-04, Paints and varnishes - Coating constancy of performance, classification and marking
materials and coating systems for exterior masonry
and concrete - Part 3: Determination of liquid water EN 12004-2
permeability EN 12004-2:2017, Adhesives for ceramic tiles - Part 2:
Test methods
EN 1062-6
EN 1062-6:2002-10, Paints and varnishes - Coating EN 13501-1
materials and coating systems for exterior masonry EN 13501-1:2018, Fire classification of construction
and concrete - Part 6: Determination of carbon dioxide products and building elements - Part 1: Classification
permeability using data from reaction to fire tests
EN 1279-4 EN 13813
EN 1279-4:2002 Glass in building - Insulating glass EN 13813:2002-10, Screed material and floor screeds
units - Part 4: Methods of test for the physical - Screed materials - Properties and requirements
attributes of edge seals
EN 13892-8
EN 1504-2 EN 13892:2003-02, Methods of test for screed
EN 1504-2:2004-12, Products and systems for the materials - Part 8: Determination of bond strength
protection and repair of concrete structures -
Definitions, requirements, quality control and ISO 14025
evaluation of conformity - Part 2: Surface protection DIN EN ISO 14025:2011-10, Environmental labels and
systems for concrete declarations — Type III environmental declarations —
Principles and procedures
EN 1504-4
EN 1504-4:2004-11, Products and systems for the EN 14891
protection and repair of concrete structures - EN 14891:2012-04, Liquid applied water impermeable
Definitions, requirements, quality control and products for use beneath ceramic tiling - Definitions,
evaluation of conformity- Part 4: Structural bonding specifications and test methods
EN 1504-5 EN 15804
EN 1504-5:2004-12, Products and systems for the EN 15804:2019+A2, Sustainability of construction
protection and repair of concrete structures - works — Environmental Product Declarations — Core
Definitions, requirements, quality control and rules for the product category of construction products
evaluation of conformity - Part 5: Concrete injection
EN 16516
EN 1542 EN 16516:2017
EN 1542:1999-07, Products and systems for the Construction products - Assessment of release of
protection and repair of concrete structures - Test dangerous substances - Determination of emissions
methods - Measurement of bond strength by pull-off into indoor air
EN 1771 EN ISO 17025
EN 1771:2004-11, Products and systems for the EN ISO 17025:2018-03
protection and repair of concrete structures - Test General requirements for the competence of testing
methods - Determination of injectability and splitting and calibration laboratories
test
EN ISO 17178
ISO 2811-1 EN ISO 17178:2020-06, Adhesives - Adhesives for
ISO 2811-1:2016, Paints and varnishes - bonding parquet to subfloor - Test methods and
Determination of density - Part 1: Pycnometer method minimum requirements
EN ISO 3219 EN 17333-2
EN ISO 3219:1994-10, Plastics - Polymers/resins in EN 17333-2:2020+AC:2020, Characterisation of one
the liquid state or as emulsions or dispersions - component foam - Part 2: Expansion characteristics
Determination of viscosity using a rotational viscometer
with defined shear rate EN 17333-3
EN 17333-3:2020, Characterisation of one component
ISO 3219-2 foam - Part 3: Application
ISO 3219-2:2021, Rheology - Part 2: General
principles of rotational and oscillatory rheometry EN 17333-4
EN 17333-4:2020, Characterisation of one component
EN ISO 7783 foam - Part 4: Mechanical strength
11 Environmental Product Declaration FEICA/EFCC/IVK/DBC – Products based on polyurethane or silane-modified polymer,
group 2
data sets http://documentation.gabi-software.com/,
EN 17333-5 2020
EN 17333-5:2020, Characterisation of one component
foam - Part 5: Insulation German AgBB
Committee for Health-related Evaluation of Building
EN ISO 22636 Products: health-related evaluation of emissions of
EN ISO 22636:2020, Adhesives - Adhesives for floor volatile organic compounds (VOC and SVOC) from
coverings - Requirements for mechanical and electrical building products; status: June 2012
performance www.umweltbundesamt.de/produkte/bauprodukte/agb
b.htm
EAD 030350-00-0402
EAD 030350-00-0402:2018-08, Liquid Applied Roof IBU 2021
Waterproofing Kits Institut Bauen und Umwelt e.V.: General Instructions
for the EPD programme of Institut Bauen und Umwelt
EAD 030352-00-0503 e.V. EPD programme. Version 2.0. Berlin: Institut
EAD 030352-00-0503:2019-01, Liquid applied Bauen und Umwelt e.V., 2021
watertight covering kits for wet room floors and/or walls www.ibu-epd.com
2000/532/EC ift-Guideline VE-08/4
Commission decision dated 3 May 2000 replacing ift-Guideline VE-08/4:2017, Beurteilungsgrundlage für
decision 94/3/EC on a waste directory in accordance geklebte Verglasungssysteme
with Article 1 a) of Council Directive 75/442/EEC on
waste and Council decision 94/904/EC on a directory Indoor Air Comfort
of hazardous waste in terms of Article 1, paragraph 4 Product certification by Eurofins, Hamburg, Germany
of Directive 91/689/EEC on hazardous waste www.eurofins.com
Belgian Royal Decree C-2014/24239 PCR Part A
Belgisch Staatsblad 8 MEI 2014, p. 60603. — Product Category Rules for Building-Related Products
Koninklijk besluit tot vaststelling van de and Services, Part A: Calculation Rules for the Life
drempelniveaus voor de emissies naar het Cycle Assessment and Requirements on the Project
binnenmilieu van bouwproducten voor bepaalde report, Version 1.1, Institut Bauen und Umwelt e.V.,
geoogde gebruiken 2021-01
Blue Angel PCR Part B
Environmental label organised by the federal Product Category Rules for Construction Products,
government of Germany www.blauer-engel.de Part B: Reaction resin products, Institut Bauen und
Umwelt e.V., 2019-01
CPR
CPR Regulation (EU) No 305/2011 of the European RAL-GZ 716
Parliament and of the Council of 9 March 2011 laying RAL-GZ 716:2019-04 part 2, Kunststoff-
down harmonised conditions for the marketing of Fensterprofilsysteme - Gütesicherung
construction products and repealing Council Directive
89/106/EEC REACH
Directive (EG) No. 1907/2006 of the European
Decopaint Directive Parliament and of the Council dated 18 December
Directive 2004/42/CE of the European Parliament and 2006 on the registration, evaluation, approval and
the council of 21 April 2004 on the limitation of restriction of chemical substances (REACH), for
emissions of volatile organic compounds due to the establishing a European Agency for chemical
use of organic solvents in certain paints and varnishes substances, for amending Directive 1999/45/EC and
and vehicle refinishing products and amending for annulment of Directive (EEC) No. 793/93 of the
Directive 1999/13/EC Council, Directive (EC) No. 1488/94 of the
Commission, Guideline 76/769/EEC of the Council and
EMICODE Guidelines 91/155/EEC, 93/67/EEC, 93/105/EC and
EMICODE, GEV – Gemeinschaft 2000/21/EC of the Commission.
Emissionskontrollierte Verlegewerkstoffe, Klebstoffe
und Bauprodukte e. V. (pub.).www.emicode.de
GaBi 10 software & documentation
Data base for Life Cycle Engineering LBP, University
of Stuttgart and Sphera, documentation of GaBi 10
12 Environmental Product Declaration FEICA/EFCC/IVK/DBC – Products based on polyurethane or silane-modified polymer,
group 2
Publisher
Institut Bauen und Umwelt e.V. Tel +49 (0)30 3087748- 0
Hegelplatz 1 Fax +49 (0)30 3087748- 29
10117 Berlin Mail info@ibu-epd.com
Germany Web www.ibu-epd.com
Programme holder
Institut Bauen und Umwelt e.V. Tel +49 (0)30 - 3087748- 0
Hegelplatz 1 Fax +49 (0)30 – 3087748 - 29
10117 Berlin Mail info@ibu-epd.com
Germany Web www.ibu-epd.com
Author of the Life Cycle
Assessment Tel +49 711 341817-0
Sphera Solutions GmbH Fax +49 711 341817-25
Hauptstraße 111- 113 Mail info@sphera.com
70771 Leinfelden-Echterdingen Web www.sphera.com
Germany
Owner of the Declaration
FEICA - Association of the Tel +32 (0)267 673 20
European Adhesive and Sealant Fax +32 (0)267 673 99
Industry Mail info@feica.eu
Avenue E. van Nieuwenhuyse 2 Web www.feica.eu
B-1160 Brussels
Belgium
Tel +32289720-39
Fax +32289720-37
EFCC - European Federation for Mail info@efcc.be
Construction Chemicals Web www.efcc.eu
Boulevard du Triomphe 172
1160 Brussels
Belgium
Tel +49 (0)69 2556-1318
Fax +49 (0)69 2556-1319
Mail info@deutsche-bauchemie.de
Deutsche Bauchemie e.V. Web www.deutsche-bauchemie.de
Mainzer Landstr. 55
60329 Frankfurt
Germany
Tel +49 (0)211 67931-10
Fax +49 (0)211 67931-33
Mail info@klebstoffe.com
Industrieverband Klebstoffe e.V Web www.klebstoffe.com
Völklinger Straße 4
40219 Düsseldorf
Germany
