ENVIRONMENTAL PRODUCT DECLARATION
as per ISO 14025 and EN 15804+A2
Owner of the Declaration Balsan
Programme holder Institut Bauen und Umwelt e.V. (IBU)
Publisher Institut Bauen und Umwelt e.V. (IBU)
Declaration number EPD-BAL-20220238-CCA1-EN
Issue date 18.08.2022
Valid to 17.08.2027
TOP DESIGN 1100 ECO
tufted carpet made of recycled material
Balsan
www.ibu-epd.com | https://epd-online.com
Umwelt Produktdeklaration Name des Herstellers – Name des Produkts
General Information
Balsan TOP DESIGN 1100 ECO - tufted
carpet made of recycled material
Programme holder Owner of the declaration
IBU – Institut Bauen und Umwelt e.V. Balsan
Hegelplatz 1 Corbilly - D14
10117 Berlin 36330 Arthon
Germany France
Declaration number Declared product / declared unit
EPD-BAL-20220238-CCA1-EN 1 m2 tufted carpet TOP DESIGN 1100 ECO
This declaration is based on the product Scope:
category rules: The manufacturer declaration applies to the tufted
Floor coverings, 02/2018 carpet TOP DESIGN 1100 ECO with the GUT-
(PCR checked and approved by the SVR) PRODIS license number 4FA9B794.
The carpet is produced in the Balsan manufacturing
sites Arthon, France.
Issue date
The declaration is only valid in conjunction with a valid
18.08.2022
GUT-PRODIS license of the product.
Valid to
The owner of the declaration shall be liable for the
17.08.2027
underlying information and evidence; the IBU shall not
be liable with respect to manufacturer information, life
cycle assessment data and evidences.
The EPD was created according to the specifications
of EN 15804+A2. In the following, the standard will be
simplified as EN 15804.
Verification
The standard EN 15804 serves as the core PCR
Independent verification of the declaration and data
according to ISO 14025:2011
Dipl. Ing. Hans Peters internally x externally
(chairman of Institut Bauen und Umwelt e.V.)
Dr. Alexander Röder Angela Schindler
(Managing Director Institut Bauen und Umwelt e.V.)) (Independent verifier)
Product
Product description/Product definition Application
TOP DESIGN 1100 ECO - tufted wall-to-wall carpet According to the use class as defined in EN 1307 the
having a surface pile of polyamide 6 with 100 % products can be used in all professional areas which
recycled content and a textile backing made of require class 33 or less.
polypropylene. The carpet is coloured by an injection
printing system, which allows the creation of various
designs.
The total recycled content amounts to 52 %.
For the placing on the market of the product in the
European Union/European Free Trade Association
(EU/EFTA) (with the exception of Switzerland)
Regulation (EU) No. 305/2011 Construction Product
Regulation (CPR) applies. The product needs a
Declaration of Performance (DoP) taking into
consideration EN 14041:2018-05, Resilient, textile and
laminate floor coverings - Essential characteristics, and
the CE-marking. The DoP of the product can be found
on the manufacturer's technical information section.
For the application and use of the product the
respective national provisions apply.
2 Environmental Product Declaration Balsan – TOP DESIGN 1100 ECO - tufted carpet
Technical Data Base materials/Ancillary materials
Name Value Unit
Constructional data Polyamide 6 51.6 %
Name Value Unit Polypropylene 9.3 %
Product Form Rolls of 4 m width - SBR-latex 7.1 %
Type of manufacture Tufted carpet - Limestone 31.9 %
Polyamide 6, Additives 0.1 %
Yarn type -
100 % recycled This product contains substances listed in the ECHA
Colouration Injection printing candidate list (10.06.2022) or other carcinogenic,
Primary backing Polypropylene mutagenic or reprotoxic (CMR) substances in
Textile backing made categories 1A or 1B which are not on the candidate list
Secondary backing -
of polypropylene exceeding 0.1 percentage by mass: no
Surface pile weight 805 g/m2 The products are registered in the GUT-PRODIS
Surface pile thickness 4.9 mm Information System. The PRODIS system ensures the
Total pile weight 1100 g/m² compliance with limitations of various chemicals and
Total carpet weight 2130 g/m2 Volatile Organic Compound (VOC)-emissions and a
Total thickness 7.5 mm ban on the use of all substances that are listed as
Number of tufts or loops 1935 pce/dm2 'Substances of Very High Concern' (SVHC) under
REACH.
Reference service life
Performance data of the product in accordance with
The service life of textile floor coverings strongly
the declaration of performance with respect to its
depends on the correct installation taking into account
essential characteristics according to EN 14041:
the declared use classification and the adherence to
2018- 05, Resilient, textile and laminate floor coverings
cleaning and maintenance instructions.
- Essential characteristics.
A calculation of the reference service life according to
Additional product properties in accordance with EN
ISO 15686 is not possible.
1307 can be found on the Product Information System
Alternatively, a reference service life of 10 years can
PRODIS using the PRODIS registration number of the
be assumed, during which the functional and visual
product (www.pro-dis.info) or on the manufacturer's
quality is guaranteed (BNB, Nutzungsdauer von
technical information section (www.balsan.com).
Bauteilen). The technical service life can be
significantly longer.
LCA: Calculation rules
Declared Unit residual waste (except radioactive waste). Benefits for
generated electricity and steam due to the incineration
of production waste are aggregated.
Name Value Unit Biogenic carbon that is stored in renewable material
Declared unit 1 m2 (packaging paper) is taken into account as well as the
Grammage 2.13 kg/m2 associated carbon dioxide uptake from the air from
Layer thickness 0.0075 m which this biogenic carbon originates.
Gross density 284 kg/m3
The declared unit refers to 1 m2 produced textile floor A4 Transport
covering. The output of module A5 'Assembly' is 1 m2 Transport of the packed textile floor covering from
installed textile floor covering. factory gate to the place of installation.
A5 Installation
System boundary Installation of the textile floor covering, processing of
Type of EPD installation waste and packaging waste up to the
Cradle-to-gate with options, module C1-C4, module D, landfill disposal of residual waste (except radioactive
and additional modules A4, A5, B1, B2 waste), the production of the amount of carpet that
occurs as installation waste including its transport to
System boundaries of modules A, B, C, D the place of installation.
Modules C3, C4 and D are indicated separately for Generated electricity and steam due to the incineration
three end-of-life scenarios: of waste are listed in the result table as exported
1 - landfill disposal energy.
2 - municipal waste incineration Biogenic carbon that is stored in renewable materials
3 - recovery in a cement plant in packaging paper is released as carbon dioxide
emissions into the air at the end of life in module A5.
A1-A3 Production Preparation of the floor and auxiliary materials
Energy supply and production of the basic material, (adhesives, fixing agents, PET connectors) are beyond
processing of secondary material, auxiliary material, the system boundaries and not taken into account.
transport of the material to the manufacturing site,
emissions, waste water treatment, packaging material
and waste processing up to the landfill disposal of
3 Environmental Product Declaration Balsan – TOP DESIGN 1100 ECO - tufted carpet
B1 Use the result table as exported energy.
Indoor emissions during the use stage. After the first C3-3: Collection of the carpet waste for recovery in the
year, no product-related Volatile Organic Compound cement industry, waste processing (granulating),
(VOC) emissions are relevant due to known VOC transport to the cement plant, emissions from the
decay curves of the product. incineration.
B2 Maintenance C4 Disposal
Cleaning of the textile floor covering for a period of 1 C4-1: Impact from landfill disposal,
year: C4-2: The carpet waste leaves the system in module
Vacuum cleaning – electricity supply C3-2,
Wet cleaning – electricity, water consumption, C4-3: The pre-processed carpet waste leaves the
production of the cleaning agent, waste water system in module C3-3.
treatment.
The declared values in this module have to be D Recycling potential
multiplied by the assumed service life of the floor Calculated benefits result from materials exclusive
covering in the building in question. secondary materials (net materials).
D-A5: Benefits for generated energy due
B3 - B5 Repair, replacement, refurbishment to incineration of packaging and installation waste
The modules are not relevant within the assumed (incineration plant with R1 > 0.6),
reference service life of 10 years. D-1: Benefits for generated energy due to landfill
disposal of carpet waste at the end of life,
B6 - B7 Operational energy and water use D-2: Benefits for generated energy due to incineration
No energy and water input are required for the of carpet waste at the end-of-life (incineration plant
operation of the carpet in the use stage. The modules with R1 > 0.6),
are not relevant and not declared D-3: Benefits for saved fossil energy and saved
inorganic material due to recovery of the carpet in a
C1 De-construction cement plant.
The floor covering is de-constructed manually and no
additional environmental impact is caused. Comparability
Basically, a comparison or an evaluation of EPD data
C2 Transport is only possible if all the data sets to be compared
Transport of the carpet waste to a landfill, to the were created according to EN 15804 and the building
municipal waste incineration plant (MWI) or to the context, respectively the product-specific
waste collection facility for recycling. characteristics of performance, are taken into account.
C3 Waste processing Background data are taken from the GaBi database,
C3-1: Landfill disposal needs no waste processing. 2022-1. Remaining data gaps are covered by the
C3-2: Impact from waste incineration (plant with ecoinvent 3.7 database, 2020.
R1>0.6), generated electricity and steam are listed in
LCA: Scenarios and additional technical information
Characteristic product properties fixing agents, PET connectors etc.) are not taken into
Information on biogenic Carbon account.
Maintenance (B2)
Name Value Unit The values for cleaning refer to 1 m2 floor covering per
Biogenic Carbon Content in year.
0.013 kg C
accompanying packaging Depending on the application based on ISO 10874, the
1 kg biogenic Carbon is equivalent to 44/12 kg of CO technical service life recommended by the
2
manufacturer and the anticipated strain on the floor by
customers, the case-specific useful life can be
established. Based on this useful life the effects of
module B2 need to be calculated in order to obtain the
Transport to the construction site (A4) overall environmental impacts.
Name Value Unit Name Value Unit
Litres of fuel 0.005 l/100km Number/
Maintenance cycle (vacuum cleaning) 208
Transport distance 700 km year
Capacity utilisation (including empty Number/
55 % Maintenance cycle (wet cleaning) 1,5
runs) year
Gross density of products transported 284 kg/m3 Water consumption (wet cleaning) 4,4 kg/year
Cleaning agent (wet cleaning) 0,09 kg/year
Installation in the building (A5) Electricity consumption 0,314 kWh/year
Name Value Unit
Material loss 0.192 kg
Polyethylene packaging waste and installation waste
are considered to be incinerated in a municipal waste
incineration plant. Cardboard packaging waste is going
to be recycled.
Preparation of the floor and auxiliaries (adhesives,
4 Environmental Product Declaration Balsan – TOP DESIGN 1100 ECO - tufted carpet
Reference service life
Name Value Unit
Life Span (according to
10 a
BBSR)
Corresponds to the
Declared product properties
specifications of -
(at the gate) and finishes
EN 1307
An assumed quality of work,
Conforms to the
when installed in
manufacturer's -
accordance with the
instructions
manufacturer’s instructions
Use in areas
Usage conditions, e.g.
corresponding to use
frequency of use, -
class 33 according to
mechanical exposure
EN 1307
Maintenance e.g. required
According to the
frequency, type and quality
manufacturers -
and replacement of
instructions
components
End of Life (C1-C4)
Three different end of life scenarios are declared and
the results are indicated separately in module C.
Each scenario is calculated as a 100% scenario.
Scenario 1: 100 % landfill disposal
Scenario 2: 100 % municipal waste incineration (MWI)
with R1 > 0.6
Scenario 3: 100 % recovery in the cement industry
If combinations of these scenarios have to be
calculated this should be done according to the
following scheme:
EOL-impact = x % impact (Scenario 1)
+ y % impact (Scenario 2)
+ z % impact (Scenario 3)
with x % + y % + z % = 100 %
Name Value Unit
Collected as mixed construction waste
2.13 kg
(scenario 1 and 2)
Collected separately (scenario 3) 2.13 kg
Landfilling (scenario 1) 2.13 kg
Energy recovery (scenario 2) 2.13 kg
Energy recovery (scenario 3) 1.45 kg
Recycling (scenario 3) 0.68 kg
Reuse, recovery and/or recycling potentials (D),
relevant scenario information
Recovery or recycling potentials due to the three end
of life scenarios (module C) are indicated separately.
Recycling in the cement industry (scenario 3)
The organic material of the carpet is used as an
alternative fuel in a cement kiln. It mainly substitutes
for lignite (68.8 %), hard coal (23.6 %) and petrol coke
(7.6 %). The inorganic material is substantially
integrated into the cement clinker and substitutes for
original material input VDZ e.V.
5 Environmental Product Declaration Balsan – TOP DESIGN 1100 ECO - tufted carpet
LCA: Results
The modules C3/1, C4/2 and C4/3 cause no additional impact (see chapter "LCA: Calculation rules").
Module C2 represents the transport for scenarios 1, 2 and 3. The values in column D result from module A5.
DESCRIPTION OF THE SYSTEM BOUNDARY (X = INCLUDED IN LCA; ND = MODULE OR INDICATOR NOT
DECLARED; MNR = MODULE NOT RELEVANT)
BENEFITS AND
CONSTRUCTI LOADS
PRODUCT STAGE ON PROCESS USE STAGE END OF LIFE STAGE BEYOND THE
STAGE SYSTEM
BOUNDARIES
6 Environmental Product Declaration Balsan – TOP DESIGN 1100 ECO - tufted carpet
lairetam
waR
ylppus tropsnarT
gnirutcafunaM
eht
morf
tropsnarT
etis
eht
ot
etag
ylbmessA esU
ecnanetniaM
riapeR
tnemecalpeR tnemhsibrufeR
ygrene
lanoitarepO esu
retaw
lanoitarepO esu
noitcurtsnoc-eD
noitilomed tropsnarT
gnissecorp
etsaW
lasopsiD -esueR -yrevoceR -gnilcyceR laitnetop
A1 A2 A3 A4 A5 B1 B2 B3 B4 B5 B6 B7 C1 C2 C3 C4 D
X X X X X X X MNR MNR MNR ND ND X X X X X
RESULTS OF THE LCA - ENVIRONMENTAL IMPACT according to EN 15804+A2: 1 m² floor covering
Core Indicator Unit A1-A3 A4 A5 B1 B2 C1 C2 C3/2 C3/3 C4/1 D D/1 D/2 D/3
GWP-total [kg CO2-Eq.] 5.11E+01.29E-1 9.15E-10.00E+04.16E-10.00E+07.23E-33.96E+03.99E+01.49E-1-6.15E-20.00E+0-4.68E-1-7.35E-2
GWP-fossil [kg CO2-Eq.] 5.31E+01.27E-1 8.87E-10.00E+02.15E-10.00E+07.10E-33.96E+03.99E+01.49E-1-6.11E-20.00E+0-4.66E-1-7.35E-2
GWP-biogenic [kg CO2-Eq.] -2.06E-11.64E-3 2.76E-20.00E+04.16E-30.00E+09.19E-5 4.31E-4 7.58E-4 1.81E-8-3.11E-40.00E+0-2.36E-3-9.29E-6
GWP-luluc [kg CO2-Eq.] 6.53E-3 7.17E-4 6.62E-40.00E+01.96E-10.00E+04.02E-5 7.24E-5 1.75E-4 7.35E-5-6.68E-60.00E+0-5.07E-5-3.53E-5
7.71E- 4.32E- 3.06E- 4.66E- 2.03E- -4.11E- -3.11E- -1.40E-
ODP [kg CFC11-Eq.] 1.29E-8 1.16E-90.00E+03.42E-80.00E+0 0.00E+0
15 16 13 13 13 13 12 13
AP [mol H+-Eq.] 1.64E-2 7.66E-4 1.98E-30.00E+08.32E-40.00E+04.29E-5 4.69E-3 4.82E-3 4.47E-4-8.01E-50.00E+0-6.09E-4-2.23E-4
EP-freshwater [kg P-Eq.] 6.17E-5 3.84E-7 5.61E-60.00E+05.19E-60.00E+02.15E-8 2.95E-7 3.81E-7 2.82E-5-8.36E-80.00E+0-6.33E-7-9.96E-8
EP-marine [kg N-Eq.] 5.87E-3 3.76E-4 7.77E-40.00E+01.97E-40.00E+02.11E-5 2.36E-3 2.42E-3 9.90E-5-2.18E-50.00E+0-1.66E-4-7.55E-5
EP-terrestrial [mol N-Eq.] 5.38E-2 4.16E-3 7.62E-30.00E+02.83E-30.00E+02.33E-4 2.64E-2 2.70E-2 1.09E-3-2.33E-40.00E+0-1.77E-3-8.28E-4
POCP [kg NMVOC-Eq.]1.46E-2 7.11E-4 1.93E-3 4.18E-4 9.83E-40.00E+03.98E-5 6.04E-3 6.15E-3 3.18E-4-6.10E-50.00E+0-4.64E-4-2.35E-4
6.03E-
ADPE [kg Sb-Eq.] 1.16E-6 1.08E-8 1.06E-70.00E+02.30E-70.00E+0 1.36E-8 1.81E-8 1.05E-8-9.18E-90.00E+0-6.97E-8-7.69E-9
10
- - -
ADPF [MJ] 8.86E+11.72E+08.30E+00.00E+05.90E+00.00E+09.63E-21.77E+02.21E+02.14E+0 0.00E+0
1.04E+0 7.92E+01.06E+1
[m³ world-Eq
WDP 6.49E+01.15E-3 6.28E-10.00E+09.99E-20.00E+06.45E-5 4.42E-1 4.45E-1-1.60E-3-6.40E-30.00E+0-4.85E-2-9.90E-3
deprived]
GWP = Global warming potential; ODP = Depletion potential of the stratospheric ozone layer; AP = Acidification potential of land and water; EP =
Caption Eutrophication potential; POCP = Formation potential of tropospheric ozone photochemical oxidants; ADPE = Abiotic depletion potential for non-
fossil resources; ADPF = Abiotic depletion potential for fossil resources; WDP = Water (user) deprivation potential
RESULTS OF THE LCA - INDICATORS TO DESCRIBE RESOURCE USE according to EN 15804+A2: 1 m²
floor covering
Indicator Unit A1-A3 A4 A5 B1 B2 C1 C2 C3/2 C3/3 C4/1 D D/1 D/2 D/3
PERE [MJ] 6.22E+1 9.77E-2 5.70E+0 0.00E+0 3.69E+0 0.00E+0 5.48E-3 2.58E-1 3.81E-1 1.76E-1 -2.84E-1 0.00E+0 -2.15E+0-8.51E-2
PERM [MJ] 5.70E-2 0.00E+0 -5.70E-2 0.00E+0 0.00E+0 0.00E+0 0.00E+0 0.00E+0 0.00E+0 0.00E+0 0.00E+0 0.00E+0 0.00E+0 0.00E+0
PERT [MJ] 6.23E+1 9.77E-2 5.64E+0 0.00E+0 3.69E+0 0.00E+0 5.48E-3 2.58E-1 3.81E-1 1.76E-1 -2.84E-1 0.00E+0 -2.15E+0-8.51E-2
PENRE [MJ] 7.63E+1 1.72E+0 8.87E+0 0.00E+0 5.90E+0 0.00E+0 9.66E-2 1.36E+1 1.40E+1 2.14E+0 -1.04E+0 0.00E+0 -7.92E+0-1.06E+1
PENRM [MJ] 1.24E+1 0.00E+0 -5.59E-1 0.00E+0 0.00E+0 0.00E+0 0.00E+0 -1.18E+1-1.18E+1 0.00E+0 0.00E+0 0.00E+0 0.00E+0 0.00E+0
PENRT [MJ] 8.87E+1 1.72E+0 8.31E+0 0.00E+0 5.90E+0 0.00E+0 9.66E-2 1.77E+0 2.21E+0 2.14E+0 -1.04E+0 0.00E+0 -7.92E+0-1.06E+1
SM [kg] 1.20E+0 0.00E+0 1.08E-1 0.00E+0 0.00E+0 0.00E+0 0.00E+0 0.00E+0 0.00E+0 0.00E+0 0.00E+0 0.00E+0 0.00E+0 3.80E-1
RSF [MJ] 0.00E+0 0.00E+0 0.00E+0 0.00E+0 0.00E+0 0.00E+0 0.00E+0 0.00E+0 0.00E+0 0.00E+0 0.00E+0 0.00E+0 0.00E+0 0.00E+0
NRSF [MJ] 0.00E+0 0.00E+0 0.00E+0 0.00E+0 0.00E+0 0.00E+0 0.00E+0 0.00E+0 0.00E+0 0.00E+0 0.00E+0 0.00E+0 0.00E+0 0.00E+0
FW [m³] 1.79E-1 1.11E-4 1.71E-2 0.00E+0 3.34E-3 0.00E+0 6.19E-6 1.04E-2 1.06E-2 2.51E-5 -2.71E-4 0.00E+0 -2.05E-3 -8.56E-4
PERE = Use of renewable primary energy excluding renewable primary energy resources used as raw materials; PERM = Use of
renewable primary energy resources used as raw materials; PERT = Total use of renewable primary energy resources; PENRE = Use of
non-renewable primary energy excluding non-renewable primary energy resources used as raw materials; PENRM = Use of non-
Caption
renewable primary energy resources used as raw materials; PENRT = Total use of non-renewable primary energy resources; SM = Use
of secondary material; RSF = Use of renewable secondary fuels; NRSF = Use of non-renewable secondary fuels; FW = Use of net fresh
water
RESULTS OF THE LCA – WASTE CATEGORIES AND OUTPUT FLOWS according to EN 15804+A2:
1 m² floor covering
Indicator Unit A1-A3 A4 A5 B1 B2 C1 C2 C3/2 C3/3 C4/1 D D/1 D/2 D/3
HWD [kg] 3.22E-3 8.25E-12 2.90E-4 0.00E+0 4.19E-5 0.00E+0 4.62E-132.89E-103.08E-103.30E-10-1.41E-100.00E+0 -1.08E-9-2.15E-11
NHWD [kg] 4.59E-1 2.47E-4 7.06E-2 0.00E+0 7.30E-3 0.00E+0 1.38E-5 3.23E-1 3.23E-1 2.12E+0 -5.24E-4 0.00E+0 -3.98E-3 -2.59E-4
RWD [kg] 1.53E-3 2.12E-6 1.43E-4 0.00E+0 3.76E-4 0.00E+0 1.19E-7 5.54E-5 8.73E-5 2.63E-5 -8.13E-5 0.00E+0 -6.16E-4 -1.55E-5
CRU [kg] 0.00E+0 0.00E+0 0.00E+0 0.00E+0 0.00E+0 0.00E+0 0.00E+0 0.00E+0 0.00E+0 0.00E+0 0.00E+0 0.00E+0 0.00E+0 0.00E+0
MFR [kg] 2.50E-2 0.00E+0 3.13E-2 0.00E+0 0.00E+0 0.00E+0 0.00E+0 0.00E+0 3.80E-1 0.00E+0 0.00E+0 0.00E+0 0.00E+0 0.00E+0
MER [kg] 0.00E+0 0.00E+0 0.00E+0 0.00E+0 0.00E+0 0.00E+0 0.00E+0 0.00E+0 0.00E+0 0.00E+0 0.00E+0 0.00E+0 0.00E+0 0.00E+0
EEE [MJ] 0.00E+0 0.00E+0 7.38E-1 0.00E+0 0.00E+0 0.00E+0 0.00E+0 7.24E+0 0.00E+0 0.00E+0 0.00E+0 0.00E+0 0.00E+0 0.00E+0
EET [MJ] 0.00E+0 0.00E+0 1.33E+0 0.00E+0 0.00E+0 0.00E+0 0.00E+0 1.30E+1 4.70E+1 0.00E+0 0.00E+0 0.00E+0 0.00E+0 0.00E+0
HWD = Hazardous waste disposed; NHWD = Non-hazardous waste disposed; RWD = Radioactive waste disposed; CRU = Components
Caption for re-use; MFR = Materials for recycling; MER = Materials for energy recovery; EEE = Exported electrical energy; EET = Exported
thermal energy
RESULTS OF THE LCA – additional impact categories according to EN 15804+A2-optional:
1 m² floor covering
Indicator Unit A1-A3 A4 A5 B1 B2 C1 C2 C3/2 C3/3 C4/1 D D/1 D/2 D/3
[Disease -6.64E-
PM 1.17E-7 4.43E-9 1.23E-8 0.00E+0 6.84E-8 0.00E+02.48E-10 1.43E-8 1.51E-8 4.30E-9 0.00E+0 0.00E+0 -8.01E-9
Incidence] 10
[kBq U235-
IRP 2.58E-1 3.11E-4 2.41E-2 0.00E+0 6.78E-2 0.00E+0 1.74E-5 8.46E-3 1.39E-2 3.89E-3 -1.38E-2 0.00E+0 0.00E+0 -1.40E-3
Eq.]
ETP-fw [CTUe] 3.83E+1 1.19E+0 3.62E+0 3.60E-3 2.69E+0 0.00E+0 6.69E-2 6.65E-1 9.19E-1 2.10E+0 -2.27E-1 0.00E+0 0.00E+0-2.03E+0
-1.05E- -2.13E-
HTP-c [CTUh] 2.59E-9 2.41E-112.39E-100.00E+06.21E-100.00E+01.35E-123.87E-114.46E-119.41E-11 0.00E+0 0.00E+0
11 11
-4.02E-
HTP-nc [CTUh] 7.86E-8 1.43E-9 7.39E-9 2.60E-11 9.46E-9 0.00E+08.02E-11 1.95E-9 2.24E-9 7.89E-9 0.00E+0 0.00E+0 -1.07E-9
10
SQP [-] ND ND ND ND ND ND ND ND ND ND ND ND ND ND
PM = Potential incidence of disease due to PM emissions; IR = Potential Human exposure efficiency relative to U235; ETP-fw = Potential
Caption comparative Toxic Unit for ecosystems; HTP-c = Potential comparative Toxic Unit for humans (cancerogenic); HTP-nc = Potential
comparative Toxic Unit for humans (not cancerogenic); SQP = Potential soil quality index
The SQP indicator is not given due to considerable uncertainties in the calculation.
The result figures given in module B2 refer to a period of 1 year because a reference service life is not declared.
They have to be multiplied by the assumed service life (in years) of the floor covering in the building under
consideration.
Disclaimer 1 – for the indicator “Potential Human exposure efficiency relative to U235”.
This impact category deals mainly with the eventual impact of low dose ionizingradiation on human health of the
nuclear fuel cycle. It does not consider effects due to possible nuclear accidents, occupational exposure nor due
to radioactive waste disposal in undergroundfacilities. Potential ionizing radiation from the soil, from radon and
from some construction materials is also not measured by this indicator.
Disclaimer 2 – for the indicators “abiotic depletion potential for non-fossil resources”, “abiotic depletion potential
for fossil resources”, “water (user) deprivation potential, deprivation-weighted water consumption”, “potential
comparative toxic unit for ecosystems”, “potential comparative toxic unit for humans – cancerogenic”, “Potential
comparative toxic unit for humans - not cancerogenic”, “potential soil quality index”.
The results of this environmental impact indicator shall be used with care as the uncertainties on these results are
high or as there is limited experience with the indicator.
References
EN 1307 DIN EN ISO 14040:2006+A1:2020 Environmental
DIN EN 1307: 2014+A1:2016+A2:2018-05: Textile management - Life cycle assessment - Principles and
floor coverings - Classification framework
EN 13501-1 ISO 14044
DIN EN 13501-1:2019-05: Fire classification of DIN EN ISO 14044:2006+A1:2018+A2:2020
construction products and building elements - Part 1: Environmental management - Life cycle assessment -
Classification using data from reaction to fire tests Requirements and guidelines
EN 14041 ISO 15686
DIN EN 14041: 2018-05: Resilient, textile and laminate ISO 15686: Buildings and constructed assets -
floor coverings - Essential characteristics Service life planning
ISO 15686-1: 2011-05: Part 1: General principles and
EN 15804 framework
DIN EN 15804:2012+A2:2019 + AC:2021, ISO 15686-2: 2012-05: Part 2: Service life prediction
Sustainability of construction works — Environmental procedures
Product Declarations — Core rules for the product ISO 15686-7: 2017-04: Part 7: Performance
category of construction products evaluation for feedback of service life data
from practice
EN 16810 ISO 15686-8: 2008-06: Part 8: Reference service life
DIN EN 16810: 2017-08: Resilient, textile and laminate and service-life estimation
floor coverings – Environmental product declarations –
Product category rules Regulation (EU) No. 305/2011
Regulation No. 305/2011 Construction Products
ISO 10874 Regulation (CPR) of the European Council and of the
DIN EN ISO 10874: 2012+A1:2021-04: Resilient, European Parliament, April 2011
textile and laminate floor coverings - Classification
General Instructions for the IBU-EPD Program
ISO 14025 General Instructions for the EPD-Program of the
DIN EN /ISO 14025:2011-10/, Environmental labels Institut Bauen und Umwelt e.V., The Preparation of
and declarations — Type III environmental Environmental Product Declarations - EPDs, version
declarations — Principles and procedures 2.0, Institut Bauen und Umwelt e.V., Berlin, January
2021, www.ibu-epd.de
ISO 14040
7 Environmental Product Declaration Balsan – TOP DESIGN 1100 ECO - tufted carpet
BNB, Nutzungsdauer von Bauteilen Part B: Requirements on the EPD for floor coverings,
Bewertungssystem Nachhaltiges Bauen (BNB), V1.2, Berlin: Institut Bauen und Umwelt e.V. (IBU),
Nutzungsdauer von Bauteilen, Bundesministerium des February 2018
Inneren, für Bau und Heimat, 24.02.2017
PRODIS
ECHA candidate list Product Information System (PRODIS) of the
Candidate List of substances of very high concern European Carpet Industry, Gemeinschaft
(SVHCs) for authorisation, 08.07.2021, European umweltfreundlicher Teppichboden e.V (GUT) and
Chemicals Agency (ECHA), Helsinki, Finland European Carpet and Rug Association
(ECRA), http://www.pro-dis.info
ecoinvent
ecoinvent, Zurich, Switzerland, database version 3.7, REACH
published September 2020 Regulation (EC) No 1907/2006 of the European
Parliament and of the Council of 18 December 2006
GaBi database concerning the Registration, Evaluation, Authorisation
GaBi Software-System and Database for Life Cycle and Restriction of Chemicals (REACH), June 2017,
Engineering, thinkstep AG, Leinfelden-Echterdingen, last update: 10.06.2022
2022-1
VDZ e.V.
PCR Part A Association of German Cement Works, Ed. Environ-
Product Category Rules for Building-Related Products mental Data of the German Cement Industry 2020
and Services Part A: Calculation Rules for the Life
Cycle Assessment and Requirements on the Project
Report according to EN 15804+A2:2019, V1.2, Berlin:
Institut Bauen und Umwelt e.V. (IBU), November 2021
PCR Part B
Product Category Rules for Building-Related Products
and Services
8 Environmental Product Declaration Balsan – TOP DESIGN 1100 ECO - tufted carpet
Publisher
Institut Bauen und Umwelt e.V. Tel +49 (0)30 3087748- 0
Hegelplatz 1 Fax +49 (0)30 3087748- 29
10117 Berlin Mail info@ibu-epd.com
Germany Web www.ibu-epd.com
Programme holder
Institut Bauen und Umwelt e.V. Tel +49 (0)30 - 3087748- 0
Hegelplatz 1 Fax +49 (0)30 – 3087748 - 29
10117 Berlin Mail info@ibu-epd.com
Germany Web www.ibu-epd.com
Author of the Life Cycle
Assessment Tel +49 (0)241 96843 410
Gemeinschaft umweltfreundlicher Fax +49 (0)241 96843 400
Teppichboden (GUT) e.V. Mail mail@gut-ev.de
Schönebergstraße 2 Web www.gut-ev.org
52068 Aachen
Germany
Owner of the Declaration
Balsan Moquette Tel +33 (0) 254 2916 00
Corbilly 2 Fax +33 (0) 254 3679 08
36330 Arthon Mail cedric.charton@balsan.com
France Web www.balsan.com
