ENVIRONMENTAL PRODUCT DECLARATION
as per ISO 14025 and EN 15804+A2
Owner of the Declaration Rubner Holding AG - S.p.A.
Publisher Institut Bauen und Umwelt e.V. (IBU)
Programme holder Institut Bauen und Umwelt e.V. (IBU)
Declaration number EPD-RUB-20230231-IBC1-EN
Issue date 27.06.2023
Valid to 26.06.2028
Cross laminated timber
Rubner Holding AG - S.p.A
www.ibu-epd.com | https://epd-online.com
1. General Information
Rubner Holding AG - S.p.A Cross laminated timber
Programme holder Owner of the declaration
IBU – Institut Bauen und Umwelt e.V. Rubner Holding AG - S.p.A.
Hegelplatz 1 Handwerkerzone 2
10117 Berlin 39030 Kiens
Germany Italy
Declaration number Declared product / declared unit
EPD-RUB-20230231-IBC1-EN 1 m³ of RUBNER cross laminated timber [CLT, XLAM] with an average
density of 461 kg/m³
This declaration is based on the product category rules: Scope:
Solid wood products, 01.08.2021 This EPD is based on a declared unit of 1 m³ of cross laminated timber
(PCR checked and approved by the SVR) (moisture of 11 % at a raw density of 461 kg/m³) produced at the RUBNER
site in Brixen (Italy).
Issue date The owner of the declaration shall be liable for the underlying information
and evidence; the IBU shall not be liable with respect to manufacturer
27.06.2023
information, life cycle assessment data and evidences.
The EPD was created according to the specifications of EN 15804+A2. In
Valid to
the following, the standard will be simplified as EN 15804.
26.06.2028
Verification
The standard EN 15804 serves as the core PCR
Independent verification of the declaration and data according to ISO
14025:2011
internally X externally
Dipl.-Ing. Hans Peters
(Chairman of Institut Bauen und Umwelt e.V.)
Florian Pronold Matthias Schulz,
(Managing Director Institut Bauen und Umwelt e.V.) (Independent verifier)
1 Environmental Product Declaration - Rubner Holding AG - S.p.A - Cross laminated timber
2. Product
Constructional data
2.1 Product description/Product definition
RUBNER cross laminated timber (RUBNER-XLAM, RUBNER- Name Value Unit
CLT) is a homogenized wood-based plate-like material that is Wood types by trade names acc. spruce, pine, larch,
-
used in engineered structural timber constructions, single family to EN 1912 Douglas fir
houses as well as in multistory buildings. RUBNER-XLAM Wood moisture acc. to ETA-
< 15 %
consists of at least three layers made from kiln-dried coniferous 18/0303
wood according to EN 1912 which are orthogonally glued
Use of wood preservatives (the Where other
together at their wide faces. Due to the multi-layer cross-
wood preservative test mark to preservative means -
sectional structure combined with the technically supported
DIN 68800-3 must be indicated) are insufficient
strength and stiffness classification of the raw materials,
Bending strength acc. to ETA-
RUBNER-XLAM is characterized by a high product quality. As a 22.6 N/mm2
18/0303
result of the industrial manufacturing process, RUBNER-XLAM
exhibits steady mechanical characteristics. In addition to flat Compressive strength parallel 21 N/mm2
standard plates, RUBNER-XLAM also includes architecturally acc. to ETA-18/0303
sophisticated shell components which are curved in space. Compressive strength
2.5 N/mm2
RUBNER-XLAM has a high dimensional stability and can be rectangular acc. to ETA-18/0303
characterized as a largely crack-minimized building material. Tensile strength parallel acc. to
14 N/mm2
ETA-18/0303
For the placing of the product on the market in the European Tensile strength rectangular acc.
Union/European Free Trade Association (EU/EFTA) (with the to ETA-18/0303 0.12 N/mm2
exception of Switzerland) the Regulation (EU) No. 305/2011
Modulus of elasticity acc. to ETA-
PCR applies. The product needs a Declaration of Performance 11550 N/mm2
18/0303
taking into consideration ETA-18/0303 and the CE-marking.
Shear strength acc. to ETA-
For the application and use, the respective national provisions 1.2 N/mm2
18/0303
apply.
Shear modulus acc. to ETA-
690 N/mm2
2.2 Application 18/0303
RUBNER-XLAM is mainly used as a structural component for depending on
buildings and bridges. Dimensional deviation geometrical mm
dimesions
2.3 Technical Data
Length < 17.5 m
The performance data of the product are in accordance with the
Declaration of Performance with respect to its essential Width < 4.3 m
characteristics according to ETA-18/0303. Height (min. - max.) 0.018 to 0.3 m
RUBNER-XLAM is produced in different strength classes. For Gross density acc. to ETA-
420 kg/m3
the strength class T14 the following applies: 18/0303
Surface quality n.r. -
Risk class acc. to DIN 68800-3 4 -
Thermal conductivity acc. to EN
0.12 W/(mK)
12664
Specific heat capacity acc. to EN
1.6 kJ/kgK
12664
Water vapor diffusion equivalent
air layer thickness acc. to ISO n.r. m
12572
Water vapour diffusion resistance
20 - 50 -
factor acc. to ISO 12572
Formaldehyde emissions acc. to
< E1 μg/m3
EN 717-1
RUBNER-XLAM is manufactured in accordance with ETA-
18/0303 from coniferous species, with priority being given to
spruce, fir, pine, larch or Douglas fir. Other coniferous species
are permissible but not typical.
RUBNER-XLAM is produced from kiln-dried coniferous wood
with an average wood moisture content of around 11 % at
delivery. For bonding, only approved modern low-emission
adhesives according to chapter 2.5 are used.
The mechanical characteristics of RUBNER-XLAM are in
accordance with strength classes specified in ETA-18/0303. For
determination of the technical specifications, the declarations of
performance (DOP) in the currently valid versions apply. The
dimensional tolerances are defined in accordance with ETA-
18/0303 and to Data Sheet XLAM.
The products are manufactured in domestic visual quality, in
2 Environmental Product Declaration - Rubner Holding AG - S.p.A - Cross laminated timber
visual-industrial quality or industrial quality according to Data To ensure the product quality, a treatment with weathering or
Sheet XLAM. wood preservatives may be required for transport to the
Use of preventive chemical wood preservatives in accordance construction site, storage, and during assembly.
with DIN 68800-3 is unusual and permitted only if other
preservative measures given in DIN 68800-2 are not sufficient
on their own. 2.7 Environment and health during manufacturing
During production, there are no negative impacts on water and
2.4 Delivery status soil. The resulting process wastewater is fed into the local
RUBNER-XLAM is produced with the dimensions according to sewage system and cleaned according to legal regulations. The
chapter 2.3 and is delivered in accordance with Data Sheet resulting exhaust air is cleaned according to the legal
XLAM in domestic visual quality, in visual-industrial quality or regulations.
industrial quality. The tolerances according to ETA-18/0303 are Noise emissions from industrial plants are reduced by structural
met. measures and comply with the legal requirements.
The production facility has an environmental management
2.5 Base materials/Ancillary materials system ISO 14001 and a quality management system ISO
RUBNER-XLAM comprises at least three orthogonally bonded 9001.
kiln-dried coniferous single layers made from The production facility has an occupational health and safety
boards/laminations according to hEN 14081. management system OHSAS 18001.
The employee protection in the manufacturing process
The following types of adhesive systems are used for bonding complies with the respective country-specific requirements,
the individual components (finger jointing and surface bonding): employees are provided with personal protective equipment.
• Melamine-urea-formaldehyde adhesives (MUF)
2.8 Product processing/Installation
• Polyurethane adhesives (PU)
RUBNER-XLAM can be processed with commercially available
tools. The instructions for occupational safety/assembly are to
RUBNER-XLAM contains the following proportions of
be observed.
ingredients per m³ on average:
• Coniferous wood (atro), mainly spruce approx. 88-90 % 2.9 Packaging
• Water approx. 9-10 %, Polyethylene foils are used in small quantities during
• Adhesive about 1 - 2.5 %, The proportions of the transportation. The use of polyethylene foils is less than 5 %
adhesives used are based on about 85 % PU and about depending on the necessity.
15 % MUF
2.10 Condition of use
The product has an average density of 461 kg/m³. The composition of RUBNER-XLAM corresponds to the
composition according to Section 2.5 for the entire period of
This product/article/at least one partial article contains use.
substances listed in the candidate list (date: 17.01.2023)
exceeding 0.1 percentage by mass: no. 2.11 Environment and health during use
Environmental protection: According to current knowledge, the
This product/article/at least one partial article contains other intended use of RUBNER-XLAM does not present any hazards
carcinogenic, mutagenic, reprotoxic (CMR) substances in or impairments to water, air and soil.
categories 1A or 1B which are not on the candidate list, Health protection: Under normal conditions of use, RUBNER-
exceeding 0.1 percentage by mass: no. XLAM is not expected to cause any damage or impairments to
health.
Biocide products were added to this construction product or it RUBNER-XLAM subsequently releases formaldehyde during its
has been treated with biocide products (this then concerns a life cycle.
treated product as defined by the (EU) Ordinance on Biocide RUBNER-XLAM bonded with PU-based adhesives has
Products No. 528/2012): no. formaldehyde emission values in the range of the untreated raw
material wood (sawn timber, by 0.004 ml/m³, Meyer, 1994,
2.6 Manufacture Testreport PB_2117078_CT, 2021, by 0.01 ppm).
RUBNER-XLAM is manufactured from sustainable sawn timber Measured against the limit value of 0.1 ml/m³ (0.124 mg/m³) of
(PEFC) sourcing from sustainable forestry. Wet sawn timber is the Reach Regulation 1907/2006/EG, the measured values in
kiln dried to a moisture content of about 11 % and subsequently accordance with EN 717-1 can be classified as low.
pre-planed. To ensure the characteristic values of the
RUBNER-XLAM, all individual boards are visually- or machine- 2.12 Reference service life
graded regarding strength and stiffness. Weak parts of planks, XLAM has been used in structural timber construction for more
which reduce the strength and stiffness properties due to the than 25 years and is very similar to RUBNER glulam with more
natural growth characteristics of wood, are cut out depending than 100 years of experience of use. In accordance with ETA-
on the grading class. The graded boards are subsequently 18/303, a service life of 50 years applies.
bonded by finger jointing to endless laminations. When used as designated, no end of durability must be
These laminations with infinite length and a thickness up to expected due to its natural durability (protection against
45 mm are subsequently planed and cut to the required length moisture). When used as designated, lifetime of RUBNER-
for further production. After applying the adhesive to the wide XLAM is equal to the duration of use of the building.
faces of boards/laminations, RUBNER-XLAM is pressed in a
2.13 Extraordinary effects
straight or curved press to at least 3-layer plate like blanks.
After curing the blanks are planed or grinded. If necessary, Fire
these single components are bonded together to composite RUBNER-XLAM is classified according to ETA-18/0303 as
plates with oversized final cross-section geometry also in follows:
combination with RUBNER glulam.
If necessary, the blanks are cut to their final complex shapes.
3 Environmental Product Declaration - Rubner Holding AG - S.p.A - Cross laminated timber
The preferred use of RUBNER-XLAM is in the form of reuse
Fire protection
based on the applicable country-specific requirements.
Name Value
If it is not re-used, it will be subjected to thermal utilization for
Building material class D the production of heat and electricity due to the high calorific
Burning droplets d0 value of approx. 16.5 MJ/kg (at a humidity of u = 12 %) in
Smoke gas development s2 compliance with the applicable country-specific requirements.
2.15 Disposal
Water If the residues are not used for any other cascading use, waste
No ingredients are washed out which could be hazardous to wood is disposed according to the applicable country-specific
water. requirements. Disposal represents a possible but unusual case.
RUBNER-XLAM is assigned to waste code 17 02 01 in the
Mechanical destruction European list of waste 2014/955/EU. (Treated cross laminated
The fracture behavior of RUBNER-XLAM is appearance typical timber is assigned to waste code 17 02 04).
for solid wood.
2.16 Further information
2.14 Re-use phase
More detailed information is available at: www.rubner.com
In the event of selective de-construction, RUBNER-XLAM can
easily be re-used after the end of the structure's service life.
3. LCA: Calculation rules
Thermal energy is provided in Brixen by district heating,
3.1 Declared Unit electricity is provided by the regional electricity grid (modelled
This EPD refers to a declared unit of 1 m³ of cross laminated with the Italian residual-mix) and RUBNER's photovoltaic
timber produced by the RUBNER group. The declared unit system.
refers to an average density of 461 kg/m³ and a wood moisture
at delivery of 11 %. Module C1 | Deconstruction and demolition
Declared unit After the removal of building components overlying the product,
the joints can simply be loosened by screwing or sawing and
Name Value Unit
lifted by cranes to the place of removal. Required energy
Declared unit 1 m3 demand can be neglected. The actual energy demand depends
Gross density 461 kg/m3 on the installation of the products and can therefore vary
Wood moisture at delivery 11 % greatly in the building context.
The analysed products represent average XLAM produced at
Module C2 | Transport to disposal
the Rubner site in Brixen (IT).
Module C2 includes the transport to waste treatment. In this
case, transport by truck over a transport distance of 50 km is
The declared unit was calculated on a volume-weighted basis.
assumed.
This EPD refers to an average product manufactured at one
site. All products undergo the same processing steps. A
Module C3 | Waste processing
possible variability is only expected due to the use of different
In Module C3, the chipping after the removal of the products is
wood species. The upstream chain for spruce is considered
considered. The wooden products and with them the material-
representative. The robustness of the declared LCA values can
inherent properties leave the product system as secondary
thus be classified as high.
combustibles in module C3.
Brixen not only produces cross laminated timber but also glued
Module C4 | Disposal
laminated timber. The allocation of product-specific material
The applied scenario declares the energetic recovery of the
and energy flows is based on physical relationships when
wooden products, therefore no environmental impacts are to be
possible. Where necessary, the allocation is based on the
expected from waste processing of the products in C4.
production volumes of each product line manufactured at
Brixen.
Module D | Benefits and loads beyond the system
boundary
3.2 System boundary
Applying an European average scenario, module D describes
The life cycle assessment of average cross laminated timber
the energetic recovery of the product at the end of life including
produced by RUBNER refers to a cradle-to-gate analysis of the
the corresponding energy substitution potentials.
environmental impacts with modules C1–C4 and module D
(A1–A3 + C + D). The following life cycle phases are part of the 3.3 Estimates and assumptions
analysis:
All assumptions are verified through detailed documentation
and correspond to the best possible representation of reality
Module A1–A3 | Production stage
based on the available data.
The production stage includes upstream burdens of raw
Background data for wood logs refer to generic data for spruce
materials (lamellae, adhesive system, etc.) and the
logs in bark derived from GaBi database. Spruce represents the
corresponding transports to the RUBNER production site in
majority of wood processed at RUBNER. The used dataset
Brixen (Italy). As the production site in Rohrbach delivers
represents an approximation for all other species.
lamellae to the other RUBNER sites, resulting environmental
Regional applicability of the used background data refers to
impacts refer to RUBNER's specific production process
average data under European or German conditions taken from
including drying. Direct emissions from drying are based on
the GaBi database. German data were used for the Italian
worst-case approximations and are included in the study.
market whenever European or regionalised average data were
Upstream emissions from the use of adhesive systems rely on
not available.
supplier-specific data.
4 Environmental Product Declaration - Rubner Holding AG - S.p.A - Cross laminated timber
according to ISO 14044.
Emissions from wood drying were included in the calculations
according to Rüter & Diederichs 2012. The representation of the main raw materials used for the
production of cross laminated timber is based on supplier-
3.4 Cut-off criteria specific primary data (lamellae, adhesive systems) leading to a
The LCA model covers all available input and output flows, high data quality.
which can be represented based on robust data and from which
a significant contribution can be expected. Data gaps are filled The technological, geographical and time-related
with conservative assumptions of average data or generic data representativeness of the database was kept in mind when
if available and are documented accordingly. selecting background data. Whenever specific data were
Only data with a contribution of less than 1 % were cut off. missing, either generic datasets or representative average data
Thus, no data were neglected, of which a substantial impact is were used instead. The implemented GaBi background
to be expected. All relevant data were collected datasets refer to the latest versions available and are carefully
comprehensively. Cutoff material and energy flows were chosen.
chosen carefully based on their expected quantitative
contribution as well as potential environmental impacts. Thus, it The assessment of the robustness of the average can be found
can be assumed that the sum of all neglected input flows does in Section 3.1.
not account for more than 5 % of the total material, water and
energy flows. Environmental impacts of machines, plant and 3.7 Period under review
infrastructure were not included. Foreground data were collected in the 2022 production year,
and the data are based on the volumes produced on an annual
3.5 Background data basis.
This study uses generic background data for the evaluation of
upstream environmental impacts from GaBi database 2022.2 3.8 Geographic Representativeness
as well as recognised literature such as Rüter & Diederichs Land or region, in which the declared product system is
2012. manufactured, used or handled at the end of the product´s
lifespan: Italy
All lamellae processed for cross laminated timber at group level
are delivered of the RUBNER RHI located in Rohrbach. Thus,
3.9 Allocation
the supply chain for lamellae input is based on primary data.
The representation of adhesives used for XLAM production is Carbon content and primary energy content of the products
based on primary data from RUBNER's suppliers. Where were assessed based on their material inherent properties
necessary, this information was complemented with estimates according to underlying physical relationships.
ensuring the completeness of the component's representation
3.10 Comparability
in the LCA.
Basically, a comparison or an evaluation of EPD data is only
3.6 Data quality possible if all the data sets to be compared were created
Data collection is based on product-specific questionnaires. It according to EN 15804 and the building context, respectively
follows an iterative process of clarifying questions via e-mail, the product-specific characteristics of performance, are taken
telephone calls or in personal/web meetings. Intensive into account.
discussions between the RUBNER group and Daxner & Merl
result in an accurate mapping of product-related material and The GaBi background database was used to calculate the LCA
energy flows. This leads to a high quality of foreground data (GaBi 10; 2022.2).
collected. Data collection relies on a consistent process
4. LCA: Scenarios and additional technical information
Characteristic product properties of biogenic carbon
End of life (C1-C4)
During tree growth, the wood assimilates carbon dioxide and
stores biogenic carbon. The carbon stored in the product is Name Value Unit
declared in the following table. Energy recovery 461 kg
Information on describing the biogenic Carbon Content at
Reuse, recovery and/or recycling potentials (D), relevant
factory gate
scenario information
Name Value Unit
Name Value Unit
Biogenic carbon content in product 205 kg C
Processing rate 100 %
Efficiency of power plant 68 %
The product reaches the end-of-waste status after removal from
the building, transport to processing and chipping of the
Installation into the building (A5) product. For the end of life of the cross laminated timber
The end of life of the product packaging is not declared in product, energy recovery as secondary fuel in a biomass power
module A5. plant is assumed. As the main sales market for the solid wood
Name Value Unit products is concentrated in the European region, plant-specific
characteristic values correspond to a European average
Packaging (polyethylene) 0.145 kg
scenario (EU). The scenario considers a reprocessing rate of
100 % for the solid wood products after removal from the
The end-of-life scenario used in this LCA study is based on the building. This assumption has to be adjusted accordingly when
following assumptions: applying the results in the building context. At the end of life of
5 Environmental Product Declaration - Rubner Holding AG - S.p.A - Cross laminated timber
the product, the equilibrium moisture is comparable to the the storage of the product before energy recovery.
moisture content at delivery. This value can vary depending on
6 Environmental Product Declaration - Rubner Holding AG - S.p.A - Cross laminated timber
5. LCA: Results
The following table contains the LCA results for a declared unit of 1 m³ of cross laminated timber produced by the RUBNER group
(461 kg/m³).
DESCRIPTION OF THE SYSTEM BOUNDARY (X = INCLUDED IN LCA; ND = MODULE OR INDICATOR NOT DECLARED; MNR =
MODULE NOT RELEVANT)
Benefits and
Construction loads beyond
Product stage Use stage End-of-life stage
process stage the system
boundaries
la ire ta m w a Ry lp p u s tro p s n a rT g n iru tc a fu n a M e h t m o rf tro p s n a rTe tis e h t o t e ta g y lb m e s s A e s U e c n a n e tn ia M ria p e R tn e m e c a lp e R tn e m h s ib ru fe R y g re n e la n o ita re p Oe s u re ta w la n o ita re p Oe s u n o itc u rts n o c -e Dn o itilo m e d tro p s n a rT g n is s e c o rp e ts a W la s o p s iD -e s u e R-y re v o c e R-g n ilc y c e Rla itn e to p
A1 A2 A3 A4 A5 B1 B2 B3 B4 B5 B6 B7 C1 C2 C3 C4 D
X X X MND MND MND MND MNR MNR MNR MND MND X X X X X
RESULTS OF THE LCA - ENVIRONMENTAL IMPACT according to EN 15804+A2: 1 m³ cross laminated timber (461 kg/m³)
Parameter Unit A1-A3 C1 C2 C3 C4 D
Global Warming Potential total (GWP-total) kg CO 2 eq -6.24E+02 0 1.46E+00 7.62E+02 0 -4.1E+02
Global Warming Potential fossil fuels (GWP-fossil) kg CO 2 eq 1.32E+02 0 1.39E+00 3.4E+00 0 -3.83E+02
Global Warming Potential biogenic (GWP-biogenic) kg CO 2 eq -7.56E+02 0 6.05E-02 7.59E+02 0 -2.73E+01
Global Warming Potential luluc (GWP-luluc) kg CO 2 eq 2.75E-01 0 9.32E-03 7.19E-04 0 -4.58E-02
Depletion potential of the stratospheric ozone layer (ODP) kg CFC11 eq 5.49E-09 0 1.36E-13 4.98E-11 0 -2.96E-09
Acidification potential of land and water (AP) mol H+ eq 5.74E-01 0 4.62E-03 7.47E-03 0 3.17E-01
Eutrophication potential aquatic freshwater (EP-freshwater) kg P eq 2.96E-03 0 4.94E-06 9.92E-06 0 -5.98E-04
Eutrophication potential aquatic marine (EP-marine) kg N eq 2.22E-01 0 2.11E-03 1.68E-03 0 6.88E-02
Eutrophication potential terrestrial (EP-terrestrial) mol N eq 2.1E+00 0 2.37E-02 1.76E-02 0 8.15E-01
Formation potential of tropospheric ozone photochemical oxidants kg NMVOC
6.98E-01 0 4.15E-03 4.53E-03 0 2.92E-01
(POCP) eq
Abiotic depletion potential for non fossil resources (ADPE) kg Sb eq 7.26E-05 0 1.39E-07 9.27E-07 0 -6.36E-05
Abiotic depletion potential for fossil resources (ADPF) MJ 1.98E+03 0 1.82E+01 6.17E+01 0 -6.62E+03
m3 world eq
Water use (WDP) 2.38E+01 0 1.55E-02 7.76E-01 0 -2.18E+01
deprived
RESULTS OF THE LCA - INDICATORS TO DESCRIBE RESOURCE USE according to EN 15804+A2: 1 m³ cross laminated
timber (461 kg/m³)
Parameter Unit A1-A3 C1 C2 C3 C4 D
Renewable primary energy as energy carrier (PERE) MJ 3.52E+03 0 1.26E+00 7.63E+03 0 -2.04E+03
Renewable primary energy resources as material utilization
MJ 7.59E+03 0 0 -7.59E+03 0 0
(PERM)
Total use of renewable primary energy resources (PERT) MJ 1.11E+04 0 1.26E+00 3.43E+01 0 -2.04E+03
Non renewable primary energy as energy carrier (PENRE) MJ 1.89E+03 0 1.82E+01 1.49E+02 0 -6.62E+03
Non renewable primary energy as material utilization (PENRM) MJ 9.31E+01 0 0 -8.68E+01 0 0
Total use of non renewable primary energy resources (PENRT) MJ 1.98E+03 0 1.82E+01 6.18E+01 0 -6.62E+03
Use of secondary material (SM) kg 0 0 0 0 0 0
Use of renewable secondary fuels (RSF) MJ 0 0 0 0 0 7.59E+03
Use of non renewable secondary fuels (NRSF) MJ 0 0 0 0 0 8.68E+01
Use of net fresh water (FW) m3 9.4E-01 0 1.45E-03 3.27E-02 0 -1.39E+00
RESULTS OF THE LCA – WASTE CATEGORIES AND OUTPUT FLOWS according to EN 15804+A2:
1 m³ cross laminated timber (461 kg/m³)
Parameter Unit A1-A3 C1 C2 C3 C4 D
Hazardous waste disposed (HWD) kg 7.08E-07 0 9.65E-11 5.34E-09 0 -8.2E-07
Non hazardous waste disposed (NHWD) kg 3.09E+00 0 2.97E-03 4.65E-02 0 2.29E-01
Radioactive waste disposed (RWD) kg 5.4E-02 0 3.39E-05 9.86E-03 0 -5.86E-01
Components for re-use (CRU) kg 0 0 0 0 0 0
Materials for recycling (MFR) kg 0 0 0 0 0 0
Materials for energy recovery (MER) kg 0 0 0 4.61E+02 0 0
Exported electrical energy (EEE) MJ 0 0 0 0 0 0
Exported thermal energy (EET) MJ 0 0 0 0 0 0
RESULTS OF THE LCA – additional impact categories according to EN 15804+A2-optional:
1 m³ cross laminated timber (461 kg/m³)
Parameter Unit A1-A3 C1 C2 C3 C4 D
Incidence of disease due to PM emissions (PM) Disease ND ND ND ND ND ND
7 Environmental Product Declaration - Rubner Holding AG - S.p.A - Cross laminated timber
incidence
Human exposure efficiency relative to U235 (IR) kBq U235 eq ND ND ND ND ND ND
Comparative toxic unit for ecosystems (ETP-fw) CTUe ND ND ND ND ND ND
Comparative toxic unit for humans (carcinogenic) (HTP-c) CTUh ND ND ND ND ND ND
Comparative toxic unit for humans (noncarcinogenic) (HTP-nc) CTUh ND ND ND ND ND ND
Soil quality index (SQP) SQP ND ND ND ND ND ND
The additional and optional impact categories according to EN 15804+A2 are not declared, as the uncertainty of these indicators is to
be classified as high.
Disclaimer 1 – for the indicator 'Potential Human exposure efficiency relative to U235'.
This impact category deals mainly with the eventual impact of lowdose ionizing radiation on human health of the nuclear fuel cycle. It
does not consider effects due to possible nuclear accidents, occupational exposure or radioactive waste disposal in underground
facilities. Potential ionizing radiation from the soil, from radon and from some construction materials is also not measured by this
indicator.
Disclaimer 2 – for the indicators 'abiotic depletion potential for non-fossil resources', 'abiotic depletion potential for fossil resources',
'water (user) deprivation potential, deprivation-weighted water consumption', 'potential comparative toxic unit for ecosystems', 'potential
comparative toxic unit for humans – cancerogenic', 'Potential comparative toxic unit for humans - not cancerogenic', 'potential soil
quality index'.
The results of this environmental impact indicator shall be used with care as the uncertainties on these results are high as there is
limited experience with the indicator.
6. LCA: Interpretation
The following interpretation contains a summary of the LCA After its use in the building, the product is assumed to be
results referenced to a declared unit of 1 m³ of cross laminated incinerated in a biomass power plant. As a result, the
timber. incorporated carbon is emitted again to the atmosphere
representing biogenic carbon dioxide emissions (module C3).
The global warming potential (GWP) of cross laminated timber
shows negative values in the production phase (modules A1– The negative values in the end-of-life (module D) result from
A3). These negative impacts result from the use of wood as raw the energetic treatment of the product. As the energy produced
material. Wood sequesters biogenic carbon during tree growth. at the biomass power plant can substitute (mainly fossil) fuels,
The sequestered carbon does not contribute to global warming an environmental net benefit is generated.
as long as it is stored in the biomass.
Potential global warming (GWP) due to the production of What's more, the electricity demand at the production site
RUBNER XLAM mainly stems from the provision of round wood (Italian residual-mix) represents a further driver of the
and associated impacts from forestry. environmental impact, especially with regard to fossil
greenhouse gas emissions.
8 Environmental Product Declaration - Rubner Holding AG - S.p.A - Cross laminated timber
The results of the previous EPD (EPD-RUB-20180060-IBB1- version due to the update of the underlying methodology
EN) are not directly comparable with the present updated according to EN 15804+A2.
7. Requisite evidence
The following evidence of environmental and health relevance For the verification of the workplace concentration of MDI
was provided. (according to EN 689), a test report is available (date 02. 5.
2016), the maximum allowed workplace concentration of 0.005
7.1 Formaldehyde mg/m³ is significantly higher than a measurement with < 0.0005
The emissions listed in section 2.11 are based on test results of mg/m³ has shown.
emission measurements in accordance with EN 717-1 at a For the verification of the workplace concentration of MDI (acc.
temperature of 23 °C, a relative humidity of 45 % and an air to EN 689), a test report is available (date 8.8 2022), the
change rate of 1.0 per hour. The test results all meet the maximum allowed workplace concentration of 0.005 mg/m³ is
requirements of emission class E1 according to EN 16351 of significantly higher than a measurement with < 0.0005 mg/m³
0.124 mg/m³. has shown.
For RUBNER-XLAM glued with PU adhesives, according to the 7.3 Fire gas toxicity
information of the manufacturer of the glue, no formaldehyde is Due to the heterogeneous structure of cross laminated timber,
added to the PU-glue during production of surface gluing; thus, combined with the non-applicability of the test standard DIN
the emissions are in the range of natural wood. According to 53436, no relevant measurement results are available, the test
2.11 a MUF adhesive is only used (if necessary) for the specimen geometry is not able to represent the real gas
manufacture of finger joints; the low mass proportion is not composition for a representative cross-section.
relevant for the overall assessment. RUBNER-XLAM bonded
with PU-based adhesives for the surface gluing has 7.4 VOC emissions
formaldehyde emission values in the range of of 0.01 ppm For the verification of VOC emissions, a test report (51005-002
(Testreport PB_2117078_CT, 2021). The test specimens were III B, 2016) of an emission analysis according to AgBB-Scheme
taken at random from production. 2015 for pure timber is available. Due to the adhesive system
used, based on supplier information, the VOC values are within
There is a test report for proof of occupational exposure the range of the natural wood. Analysis was performed in
(according to EN 689 (date 8. 8 2022), the maximum allowed accordance with ISO 16000-3 and ISO 16000-6.
workplace concentration of 0.369 mg/m³ is significantly higher
VOC emissions
than the measured with concentration of 0.12 mg/m³ have
Name Value Unit
shown.
TVOC (C6 - C16) acc. to AgBB 2015 10 μg/m3
7.2 MDI Sum SVOC (C16 - C22) acc. to AgBB 2015 < 5 μg/m3
When gluing RUBNER-XLAM with MDI-based adhesive, the
R (dimensionless) acc. to AgBB 2015 0.086 -
contained MDI will react completely. Thus, a MDI emission from
VOC without NIK acc. to AgBB 2015 <5 μg/m3
the finished RUBNER-XLAM is not possible. As there is no
standardised measurement process defined in test standards, Carcinogenic Substances <1 μg/m3
no test reports are available.
8. References
Standards EN 1912
EN 1912:2013-10-15, Structural timber - Strength classes -
DIN 53436 Assignment of visual grades and species.
DIN 53436:2015, Generation of thermal decomposition
products from materials for their analytic-toxicological testing. EN 12664
EN 12664:2001, Thermal performance of building materials and
DIN 68800-2 products - Determination of thermal resistance by means of
DIN 68800-2:2012-02, Wood preservation – Part 2: Preventive guarded hot plate and heat flow meter methods - Dry and moist
constructional measures in buildings. products with medium and low thermal resistance.
DIN 68800-3 EN 15804
DIN 68800-3:2012-02, Wood preservation – Part 3: Preventive DIN EN 15804:2012+A2:2019+AC:2021, Sustainability of
protection of wood with wood preservatives. construction works Environmental product declarations Core
rules for the product category of construction products.
EN 338
DIN EN 338:2016-07, Structural timber - Strength classes. EN 16351
ÖNORM EN 16351:2015-11-15, Timber structures - Cross
EN 689 laminated timber – Requirements (not harmonized in EU).
EN 689:1995, Workplace atmospheres - Guidance for the
assessment of exposure by inhalation to chemical agents for ETA-18/0303
comparison with limit values and measurement strategy. ETA-18/0303-2022, Rubner XLAM , Rubner Holding AG.
EN 717-1 hEN 14081
DIN EN 717-1:2005-01, Wood-based panels – Determination of hEN 14081-1:2016-06-01, Timber structures - Strength graded
Formaldehyde release – Part 1: Formaldehyde emission by the structural timber with rectangular cross section - Part 1:
chamber method. General requirements.
9 Environmental Product Declaration - Rubner Holding AG - S.p.A - Cross laminated timber
ISO 9001 IBU 2021
EN ISO 9001:2015, Quality management systems - Institut Bauen und Umwelt e.V.: General Programme
Requirements. Instructions for the Preparation of EPDs at the Institut Bauen
und Umwelt e.V. (IBU). Version 2.0, Berlin: Institut Bauen und
ISO 12572 Umwelt e.V., 2021. www.ibuepd.com
EN ISO 12572:2016, Hygrothermal performance of building
materials and products - Determination of water vapour Meyer, 1994
transmission properties - Cup method. Meyer, B, Boehme, C: 1994, Formaldeyhdabgabe von natürlich
gewachsenem Holz, Holzzentralblatt 122 (Formaldeyhd release
ISO 14001 of naturally grown wood), S. 1969-1972.
EN ISO 14001:2015, Environmental management systems -
Requirements with guidance for use. Ordinance on Biocide Products
Regulation (EU) No 528/2012 of the European Parliament and
ISO 14025 of the Council of 22 May 2012 concerning the making available
DIN EN ISO 14025:2011-10, Environmental labels and on the market and use of biocidal products.
declarations Type III environmental declarations Principles and
procedures. PCR part A
Product category rules for building-related products and
ISO 14044 services. Part A: Calculation Rules for the Life Cycle
DIN EN ISO 14044:2006-10, Environmental management - Life Assessment and Requirements on the Project Report according
cycle assessment - Requirements and guidelines. to EN 15804+A2:2019. Version 1.3. Berlin: Institut Bauen und
Umwelt e.V., 2022.
ISO 16000-3
ISO 16000-3:2011, Indoor air - Part 3: Determination of PCR: Solid wood products
formaldehyde and other carbonyl compounds in indoor air and Product category rules for building-related products and
test chamber air - Active sampling method. services. Part B: EPD requirements for solid wood products.
Version v2, Berlin: Institut Bauen und Umwelt e.V., 31.05.2023.
ISO 16000-6
ISO 16000-6:2011, Indoor air - Part 6: Determination of volatile PCR 305/2011 (EU)
organic compounds in indoor and test chamber air by active REGULATION (EU) No 305/2011 OF THE EUROPEAN
sampling on Tenax TA® sorbent, thermal desorption and gas PARLIAMENT AND OF THE COUNCIL of 9 March 2011 laying
chromatography using MS or MS-FID. down harmonised conditions for the marketing of construction
products and repealing Council Directive 89/106/EEC.
OHSAS 18001
OHSAS 18001:2018, Occupational Health- and Safety Rüter & Diederichs 2012
Assessment Series. Ökobilanz-Basisdaten für Bauprodukte aus Holz. Work report
from the Institut für Holztechnologie und Holzbiologie Nr.
2012/1. Hamburg: Johann Heinrich von Thünen-Institut.
Further references
1907/2006/EG
AgBB-Scheme 2015 VERORDNUNG (EG)
German Committee for HealthRelated Evaluation of Building Nr. 1907/2006 DES EUROPÄISCHEN PARLAMENTS UND
Products (AgBB): Approach to health assessment of emissions DES RATES vom 18. Dezember 2006 zur Registrierung,
of volatile organic compounds (VOCs and SVOCs) from Bewertung, Zulassung und Beschränkung chemischer Stoffe
building products. (REACH).
Candidate List 2005/610/EG
List of substances of very high concern considered for approval 2005/610/EG, COMMISSION DECISION of 9 August 2005
(status 17.01.2023) according to Article 59 para. 10 of the establishing the classes of reaction-to-fire performance for
REACH Regulation. European Chemicals Agency. certain construction products.
Data Sheet XLAM 2014/955/EU
Data Sheet – Cross laminated timber der Studiengemeinschaft 2014/955/EU,COMMISSION DECISION of 18 December 2014
Holzleimbau e.V., 2023. amending Decision 2000/532/EC on the list of waste pursuant
to Directive 2008/98/EC of the European Parliament and of the
GaBi Council.
GaBi 10, Software-System and Database for Life Cycle
Engineering. 2022.2. Stuttgart, Echterdingen: Sphera, 1992-
2022. Available at: https://sphera.com/product-sustainability-
gabi-data-search/
10 Environmental Product Declaration - Rubner Holding AG - S.p.A - Cross laminated timber
Publisher
Institut Bauen und Umwelt e.V. +49 (0)30 3087748- 0
Hegelplatz 1 info@ibu-epd.com
10117 Berlin www.ibu-epd.com
Germany
Programme holder
Institut Bauen und Umwelt e.V. +49 (0)30 3087748- 0
Hegelplatz 1 info@ibu-epd.com
10117 Berlin www.ibu-epd.com
Germany
Author of the Life Cycle Assessment
Daxner & Merl GmbH +43 676 849477826
Schleifmühlgasse 13/24 office@daxner-merl.com
1040 Wien www.daxner-merl.com
Austria
Owner of the Declaration
Rubner Holding AG - S.p.A. 0039 0474 563 777
Handwerkerzone 2 info@rubner.com
39030 Kiens www.rubner.com
Italy
11 Environmental Product Declaration - Rubner Holding AG - S.p.A - Cross laminated timber
