ENVIRONMENTAL PRODUCT DECLARATION
as per ISO 14025 and EN 15804+A2
Owner of the Declaration KONE Corporation
Publisher Institut Bauen und Umwelt e.V. (IBU)
Programme holder Institut Bauen und Umwelt e.V. (IBU)
Declaration number EPD-KON-20230578-CBA2-EN
Issue date 22.12.2023
Valid to 29.06.2028
UniDrive 20
KONE
www.ibu-epd.com | https://epd-online.com
General Information
KONE UniDrive 20
Programme holder Owner of the declaration
IBU – Institut Bauen und Umwelt e.V. KONE Corporation
Hegelplatz 1 Keilasatama 3
10117 Berlin 02150 ESPOO
Germany Finland
Declaration number Declared product / declared unit
EPD-KON-20230578-CBA2-EN 1 piece of the product: Automatic Sliding Door Operator UniDrive 20,
consisting of the following items:
• UniDrive 20 Sliding Door Operator
• Product packaging
This declaration is based on the product category rules: Scope:
Drive systems for automatic doors and gates, 01.08.2021 This Environmental Product Declaration refers to a specific sliding door
(PCR checked and approved by the SVR) operator - UniDrive 20. The production site is located in Germany. Green
electricity is being used at this production site.
Issue date Data represents the year 2022.
22.12.2023
The owner of the declaration shall be liable for the underlying information
and evidence; the IBU shall not be liable with respect to manufacturer
information, life cycle assessment data and evidences.
Valid to
29.06.2028 The EPD was created according to the specifications of EN 15804+A2. In
the following, the standard will be simplified as EN 15804.
Verification
The standard EN 15804 serves as the core PCR
Independent verification of the declaration and data according to ISO
14025:2011
internally X externally
Dipl.-Ing. Hans Peters
(Chairman of Institut Bauen und Umwelt e.V.)
Florian Pronold Dr.-Ing. Wolfram Trinius,
(Managing Director Institut Bauen und Umwelt e.V.) (Independent verifier)
1 Environmental Product Declaration - KONE - UniDrive 20
Product
Performance data of the product with respect to its
Product description/Product definition characteristics in accordance with the relevant technical
The automatic sliding door operator is a solution for any fields provision which can be applied are mentioned above.
of application and scope of operation. The UniDrive 20 allows
KONE to supply a drive system that covers all applications due Base materials/Ancillary materials
to its modular construction with a low number of components. The major material composition including the packaging of the
For the use and application of the product the respective product is listed below:
national provisions at the place of use apply. For UniDrive 20 Name Value Unit
the standards which can be applied are the following:
Aluminium 41 %
• EN 18650 Steel 26 %
• EN 16005
Electronics 14 %
• EN 60335
Paper 12 %
• EN 61000
• ISO 13849 Plastic 7 %
• Machinery Directive 2006/42/EC
The product includes partial articles which contain substances
• 2011/65/EU ROHS3 Directive
listed in the Candidate List of REACH Regulation
1907/2006/EC (date: 17.01.2023) exceeding 0.1 percentage by
The CE marking takes into account the proof of conformity with
mass: yes
the respective harmonized standards based on the legal
provisions above. • Lead (Pb): 7439-92-1 (CAS-No) is included in the
battery and some of the alloys used. The concentration
Application
in each individual alloy does not exceed 4.0% (by
The automatic sliding door operator UniDrive 20 is used as a
mass).
drive for automating sliding door systems as well as escape
and rescue routes. Applications are available for single- and
The Candidate List can be found on the ECHA website
double leaf doors.
address: https:echa.europa.eu/de/home.
Technical Data
The UniDrive 20 has following technical properties:
Name Value Unit
Height maximum 150 mm
Installation depth 180 mm
Reference service life
Opening and closing force maximum 150 N
The reference service life for the UniDrive 20 amounts to 10
Opening speed maximum 70 cm/s
years and depends on the application and frequency of use.
Closing speed maximum 50 cm/s
For repairs and renewals, suitable spare parts are available.
Hold open time maximum 180 s The sliding door operators are tested and certified EN 16005,
Supply voltage, frequency maximum 60 Hz meaning they are designed to withstand a minimum of
Class of protection 20 IP 1.000.000 cycles.
LCA: Calculation rules
Construction stage - Modules A4-A5
Declared Unit The construction process stage includes:
The declared unit is 1 piece of the product: UniDrive 20 — A4, transport to the building site;
Name Value Unit — A5, installation into the building;
Declared unit 1 pce. including provision of all materials, products and
energy, as well as waste processing up to the end-of waste
Mass of declared product 40,41 kg
state or disposal of final residues during the construction
process stage.
System boundary
Use stage - Module B6
The type of EPD is: cradle to gate with options,
The use stage related to the operation of the building
modules C1–C4, and module D (A1–A3 + C + D and
includes:
additional modules: A4 + A5 + B6)
— B6, operational energy use
Production - Module A1-A3
End-of-life stage– Modules C1-C4 and D
The product stage includes:
The end-of-life stage includes:
— A1, raw material extraction, processing and
— C1, de-construction, demolition:
mechanical treatments, processing of secondary
— C2, transport to waste processing;
material input (e.g. recycling processes),
— C3, waste processing for reuse, recovery and/or
— A2, transport to the manufacturer,
recycling;
— A3, manufacturing and assembly including provision
— C4, disposal;
of all materials, products and energy, as well as waste
including provision and all transport, provision of all
processing up to the end-of waste state.
materials, products and related energy and water use.
Module D (Benefits and loads beyond the system
2 Environmental Product Declaration - KONE - UniDrive 20
boundary) includes:
— D, recycling potentials, expressed as net impacts Comparability
and benefits. Basically, a comparison or an evaluation of EPD data is only
possible if all the data sets to be compared were created
Geographic Representativeness according to EN 15804 and the building context, respectively
Land or region, in which the declared product system is the product-specific characteristics of performance, are taken
manufactured, used or handled at the end of the product´s into account. Background database: GaBi, SP40
lifespan: Germany
LCA: Scenarios and additional technical information
Operational energy use (B6)
Characteristic product properties of biogenic carbon
Name Value Unit
Name ValueUnit Electricity consumption for 1 year 189.29 kWh
kg Days per year in use 365 days
Biogenic carbon content in product 0.276
C Active state (hours/day) 1.8 h
Biogenic carbon content in accompanying kg Idle state (hours/day) 22.2 h
1.569
packaging C Electrical power active state 14.31 W
Note: 1 kg of biogenic carbon is equivalent to 44/12 kg of CO . Electrical power idle state 22.2 W
2
End of life (C1-C4)
C1: The product dismantling from the building is done manually
without environmental burden.
Name Value Unit
Transport to the building site (A4)
Collected separately waste type 36.2 kg
Name Value Unit
Recycling 32.2 kg
Litres of fuel (per 1 kg) 0.00276 l/100km
Energy recovery 2.75 kg
Capacity utilisation (including empty runs) 55 %
Landfilling 1.17 kg
Transport distance via medium truck 100 km
Transport to waste management 50 km
The product is transported via truck and ship. The product is
stored in a logistic center in Germany. The main distribution The product is disassembled in a recycling process.
region is Europe. In order to allow scaling to a specific point of Material recycling is then assumed for the metals and
installation 100 km are declared. electronics. The plastic components are assumed to be
incinerated with energy recovery. Electromechanics and minor
proportions of residues arising from the recycling process are
Installation into the building (A5)
landfilled. Region for the End of Life is: Global.
Name Value Unit
Waste packaging (paper and plastic) 4,26 kg
Reuse, recovery and/or recycling potentials (D), relevant
scenario information
Reference service life Name Value Unit
Recycling 100 %
Name Value Unit
Life Span according to the manufacturer 10 a The collection rate is 100%.
3 Environmental Product Declaration - KONE - UniDrive 20
LCA: Results
DESCRIPTION OF THE SYSTEM BOUNDARY (X = INCLUDED IN LCA; MND = MODULE OR INDICATOR NOT DECLARED; MNR
= MODULE NOT RELEVANT)
Benefits and
Construction loads beyond
Product stage Use stage End of life stage
process stage the system
boundaries
la ire ta m w a Ry lp p u s tro p s n a rT g n iru tc a fu n a M e h t m o rf tro p s n a rTe tis e h t o t e ta g y lb m e s s A e s U e c n a n e tn ia M ria p e R tn e m e c a lp e R tn e m h s ib ru fe R y g re n e la n o ita re p Oe s u re ta w la n o ita re p Oe s u n o itc u rts n o c -e Dn o itilo m e d tro p s n a rT g n is s e c o rp e ts a W la s o p s iD -e s u e R-y re v o c e R-g n ilc y c e Rla itn e to p
A1 A2 A3 A4 A5 B1 B2 B3 B4 B5 B6 B7 C1 C2 C3 C4 D
X X X X X MND MND MNR MNR MNR X MND X X X X X
RESULTS OF THE LCA - ENVIRONMENTAL IMPACT according to EN 15804+A2: 1 piece UniDrive 20
Parameter Unit A1-A3 A4 A5 B6 C1 C2 C3 C4 D
GWP-total kg CO 2 eq 2.17E+02 3.53E-01 6.04E+00 7.66E+02 0 1.57E-01 8.36E+00 6.4E-02 -1.19E+02
GWP-fossil kg CO 2 eq 2.24E+02 3.38E-01 1.51E-01 7.62E+02 0 1.5E-01 7.01E+00 6.3E-02 -1.18E+02
GWP-biogenic kg CO 2 eq -7.59E+00 1.6E-02 5.89E+00 2.54E+00 0 7E-03 1.34E+00 2.17E-04 -3.48E-01
GWP-luluc kg CO 2 eq 1.4E-01 8.04E-06 9.94E-05 1.1E+00 0 3.58E-06 4.08E-04 1.83E-04 -2E-02
ODP kg CFC11 eq 4.11E-09 3.57E-17 1.09E-15 1.68E-11 0 1.59E-17 3.69E-15 2.35E-16 -8.15E-10
AP mol H+ eq 1.01E+00 3.38E-04 2E-03 1.68E+00 0 1.51E-04 1E-03 4.55E-04 -4.59E-01
EP-freshwater kg P eq 4.13E-04 7.23E-08 2.13E-07 2E-03 0 3.22E-08 5.87E-07 1.09E-07 -6.35E-05
EP-marine kg N eq 1.44E-01 1.08E-04 6.11E-04 3.74E-01 0 4.79E-05 3.44E-04 1.17E-04 -5.8E-02
EP-terrestrial mol N eq 1.55E+00 1E-03 8E-03 3.93E+00 0 5.32E-04 7E-03 1E-03 -6.23E-01
kg NMVOC
POCP 4.51E-01 3.04E-04 2E-03 1.02E+00 0 1.35E-04 9.49E-04 3.55E-04 -1.89E-01
eq
ADPE kg Sb eq 6.4E-03 1.01E-08 1.72E-08 2.21E-04 0 4.51E-09 5.1E-08 5.7E-09 -3E-03
ADPF MJ 2.9E+03 4.79E+00 1.91E+00 1.34E+04 0 2.13E+00 3.53E+00 8.32E-01 -1.64E+03
m3 world eq
WDP 3.61E+01 6.62E-04 7.49E-01 1.66E+02 0 2.95E-04 8.56E-01 7E-03 -6.45E+00
deprived
GWP = Global warming potential; ODP = Depletion potential of the stratospheric ozone layer; AP = Acidification potential of land and water; EP =
Eutrophication potential; POCP = Formation potential of tropospheric ozone photochemical oxidants; ADPE = Abiotic depletion potential for non-fossil
resources; ADPF = Abiotic depletion potential for fossil resources; WDP = Water (user) deprivation potential)
RESULTS OF THE LCA - INDICATORS TO DESCRIBE RESOURCE USE according to EN 15804+A2: 1 piece UniDrive 20
Parameter Unit A1-A3 A4 A5 B6 C1 C2 C3 C4 D
PERE MJ 1.06E+03 1.5E-02 5.15E+01 5.94E+03 0 7E-03 9.9E+00 1.09E-01 -7.04E+02
PERM MJ 6.01E+01 0 -5.11E+01 0 0 0 -9E+00 0 0
PERT MJ 1.12E+03 1.5E-02 3.47E-01 5.94E+03 0 7E-03 8.97E-01 1.09E-01 -7.04E+02
PENRE MJ 2.83E+03 4.8E+00 1.91E+00 1.34E+04 0 2.13E+00 7.69E+01 8.32E-01 -1.64E+03
PENRM MJ 7.34E+01 0 0 0 0 0 -7.34E+01 0 0
PENRT MJ 2.91E+03 4.8E+00 1.91E+00 1.34E+04 0 2.13E+00 3.53E+00 8.32E-01 -1.64E+03
SM kg 3.26E+00 0 0 0 0 0 0 0 0
RSF MJ 0 0 0 0 0 0 0 0 0
NRSF MJ 0 0 0 0 0 0 0 0 0
FW m3 2.5E+00 2.71E-05 1.8E-02 6.87E+00 0 1.21E-05 2E-02 2.1E-04 -1.27E+00
PERE = Use of renewable primary energy excluding renewable primary energy resources used as raw materials; PERM = Use of renewable primary
energy resources used as raw materials; PERT = Total use of renewable primary energy resources; PENRE = Use of non-renewable primary energy
excluding non-renewable primary energy resources used as raw materials; PENRM = Use of non-renewable primary energy resources used as raw
materials; PENRT = Total use of non-renewable primary energy resources; SM = Use of secondary material; RSF = Use of renewable secondary fuels;
NRSF = Use of non-renewable secondary fuels; FW = Use of net fresh water
RESULTS OF THE LCA – WASTE CATEGORIES AND OUTPUT FLOWS according to EN 15804+A2:
1 piece UniDrive 20
Parameter Unit A1-A3 A4 A5 B6 C1 C2 C3 C4 D
HWD kg 3.01E-05 4.65E-10 2.81E-09 5.55E-06 0 2.07E-10 1.26E-08 1.27E-08 -1.53E-05
NHWD kg 4.41E+01 4.9E-04 1.89E-01 9.51E+00 0 2.18E-04 7.36E-01 4.18E+00 -2.64E+01
RWD kg 1.44E-01 5.15E-06 1E-04 2.03E+00 0 2.29E-06 1.37E-04 9.47E-06 -1.7E-01
CRU kg 0 0 0 0 0 0 0 0 0
MFR kg 0 0 0 0 0 0 2.83E+01 0 0
MER kg 0 0 0 0 0 0 0 0 0
EEE MJ 0 0 9.14E+00 0 0 0 1.5E+01 0 0
EET MJ 0 0 1.66E+01 0 0 0 3.34E+01 0 0
4 Environmental Product Declaration - KONE - UniDrive 20
HWD = Hazardous waste disposed; NHWD = Non-hazardous waste disposed; RWD = Radioactive waste disposed; CRU = Components for re-use;
MFR = Materials for recycling; MER = Materials for energy recovery; EEE = Exported electrical energy; EET = Exported thermal energy
RESULTS OF THE LCA – additional impact categories according to EN 15804+A2-optional:
1 piece UniDrive 20
Parameter Unit A1-A3 A4 A5 B6 C1 C2 C3 C4 D
Disease
PM 1.05E-05 1.78E-09 9.37E-09 1.41E-05 0 7.91E-10 1.69E-08 5.63E-09 -6.96E-06
incidence
IR kBq U235 eq 2.71E+01 7.36E-04 1.6E-02 3.34E+02 0 3.27E-04 1.3E-02 9.75E-04 -3.4E+01
ETP-fw CTUe 1.06E+03 3.4E+00 9.05E-01 5.73E+03 0 1.51E+00 1.34E+00 4.75E-01 -5.7E+02
HTP-c CTUh 2.76E-07 6.39E-11 4.79E-11 1.58E-07 0 2.84E-11 1.14E-10 7.04E-11 -2.45E-08
HTP-nc CTUh 2.94E-06 2.73E-09 2.07E-09 5.83E-06 0 1.22E-09 1.1E-08 7.76E-09 -9.43E-07
SQP SQP 1.23E+03 1.2E-02 5.06E-01 4.27E+03 0 5E-03 1.05E+00 1.73E-01 -5.8E+01
PM = Potential incidence of disease due to PM emissions; IR = Potential Human exposure efficiency relative to U235; ETP-fw = Potential comparative
Toxic Unit for ecosystems; HTP-c = Potential comparative Toxic Unit for humans (cancerogenic); HTP-nc = Potential comparative Toxic Unit for humans
(not cancerogenic); SQP = Potential soil quality index
Disclaimer 1 – for the indicator 'Potential Human exposure efficiency relative to U235'. This impact category deals mainly with the
eventual impact of low-dose ionizing radiation on human health of the nuclear fuel cycle. It does not consider effects due to possible
nuclear
accidents, occupational exposure or radioactive waste disposal in underground facilities. Potential ionizing radiation from the soil,
radon and from some construction materials is also not measured by this indicator.
Disclaimer 2 – for the indicators 'abiotic depletion potential for non-fossil resources', 'abiotic depletion potential for fossil resources',
'water (user) deprivation potential, deprivation-weighted water consumption', 'potential comparative toxic unit for ecosystems', 'potential
comparative toxic unit for humans –
cancerogenic', 'Potential comparative toxic unit for humans - not cancerogenic', 'potential soil quality index'. The results of this
environmental impact indicator shall be used with care as the uncertainties on these results are high as there is limited experience with
the indicator.
This EPD was created using a software tool.
References
EN 18650
EN 186501: 2010, Powered pedestrian doors Part 1: ROHS3 Directive
Product requirements and test methods Directive 2011/65/EU of the European Parliament and of the
Council of 8 June 2011 on the restriction of the use of certain
EN 18650 hazardous substances in electrical and electronic equipment
EN 186502: 2010, Powered pedestrian doors Part 2:
Safety at powered pedestrian doors Further References
EN 16005 IBU 2021
EN 16005: 2013-01, Power operated pedestrian doorsets General Instructions for the EPD programme of Institut Bauen
Safety in use - Requirements and test methods und Umwelt e.V. Version 2.0, Berlin: Institut Bauen
und Umwelt e.V., 2021. www.ibu-epd.com
EN 60335
EN 60335-1, -2-103:2020 08, Household and GaBi
similar electrical appliances - Safety - Part 1: General Sphera Solutions GmbH
requirements Gabi Software System and Database for Life Cycle
Engineering 1992-2020
EN 61000 Version 10.0.0.71
EN 61000 -1-2: 2017-07, Electromagnetic University of Stuttgart
compatibility (EMC) - Part 1-2: General Methodology Leinfelden-Echterdingen
for the achievement of functional safety of electrical
and electronic systems including equipment with GaBi ts documentation
regard to electromagnetic phenomena GaBi life cycle inventory data documentation
(https://www.gabisoftware.
ISO 13849 com/support/gabi/gabidatabase-
ISO 138491: 2021-08, Safety of machinery 2020-lci-documentation/).
Safety-related parts of control systems - Part 1:
General principles for design LCA-tool dormakaba
LCA tool, ENS (drive system)
Machinery Directive LCA-Tool No.: IBU-DOR-202108-LT1-EN
Directive 2006/42/EC of the European Parliament and Developed by Sphera Solutions GmbH.
of the Council on machinery, and amending
Directive 95/16/EC PCR Part A
PCR – Part A: Calculation Rules for the Life Cycle
REACH Assessment
Regulation (EC) No 1907/2006 of the European Parliament and and Requirements on the Project Re-port
of the Council on the Registration, Evaluation, Authorisation according to EN 15804+A2:2019, Version 1.0, Institut
and Restriction of Chemicals (REACH) Bauen und Umwelt e.V., www.ibu-epd.com.
5 Environmental Product Declaration - KONE - UniDrive 20
Bauen und
PCR Part B Umwelt e.V., www.ibu-epd.com.
PCR – Part B: Requirements on the EPD for
Drive systems for automatic doors and gates, 08. 2021, Institut
6 Environmental Product Declaration - KONE - UniDrive 20
Publisher
Institut Bauen und Umwelt e.V. +49 (0)30 3087748- 0
Hegelplatz 1 info@ibu-epd.com
10117 Berlin www.ibu-epd.com
Germany
Programme holder
Institut Bauen und Umwelt e.V. +49 (0)30 3087748- 0
Hegelplatz 1 info@ibu-epd.com
10117 Berlin www.ibu-epd.com
Germany
Author of the Life Cycle Assessment
dormakaba International Holding GmbH +49 2333 793-0
DORMA Platz 1 info.de@dormakaba.com
58256 Ennepetal www.dormakaba.com
Germany
Owner of the Declaration
KONE Corporation +358(0)204 75 1
Keilasatama 3 contact@kone.com
02150 ESPOO www.kone.com
Finland
7 Environmental Product Declaration - KONE - UniDrive 20
