Environmental Product
Declaration
as per ISO 14025 and EN 15804+A2
Owner of the declaration: AS BMGS
Publisher: Kiwa-Ecobility Experts
Program operator: Kiwa-Ecobility Experts
Registration number: EPD-BMGS-209-EN
Issue date: 24-05-2022
Valid to: 23-05-2027
Hollow core slabs
1. General information
AS BMGS Precast concrete elements
Programme operator Owner of the declaration
Kiwa-Ecobility Experts AS BMGS
Kiwa GmbH Tvaika iela 27
Voltastr. 5 LV-1005 Riga
13355 Berlin Latvia
Germany
Declaration number Declared product / declared unit
EPD-BMGS-209-EN 1 ton of precast concrete element
This declaration is based on the Product Scope
Category Rules The average EPD (type: Cradle to gate with op-
PCR B - Product Category Rules for concrete tions, modules C1-C4 and module D (A1-A5, C,
and concrete elements; German version D) is about custom made precast concrete el-
EN 16757:2017 ement - Hollow core slab, manufactured in
Riga, Latvia. The calculation is based on 1 ton
Issue date of precast concrete element with a share of
24.05.2022 1,4 m% reinforcing steel.
Kiwa-Ecobility Experts shall not be liable with
Valid to respect to manufacturer information, life cy-
23.05.2027 cle assessment data and evidence.
Verification
The standard EN 15804+A2:2019 serves as the
core PCR
Independent verification of the declaration
and data according to ISO 14025:2011-10
☐internally ☒externally
Frank Huppertz
(Head of Kiwa-Ecobility Experts)
Prof. Dr. Frank Heimbecher Max Sonnen
(Chairman of the independent expert committee - (External verifier – Ecomatters)
Ecobility Experts)
Page | 2 AS BMGS - Precast concrete hollow core slab
2. Product
2.1 Product description
The product is precast concrete hollow core slab in which the reinforcing steel constitutes the main
reinforcement of the composite slab. The product is produced in various sizes (incl. thicknesses) and
applications with concrete compressive strength class of C40/50 to C50/60.
2.2 Application
The product precast concrete hollow core slab is intended to be used as wall or floor element for in-
ternal and external wall and floor constructions (including residential as well as non-residential build-
ings).
2.3 Placing on the market / Application rules
The harmonized standard EN 13369 (Common rules for precast concrete products) and product-spe-
cific standard EN 1168 (Precast concrete products - Hollow core slabs) apply for production of the
product. The CE mark is applied to the finished products.
Additional certifications: the production of AS BMGS of reinforced concrete elements is certified in
accordance with the requirements of management system standards ISO 9001:2015, ISO 14001:2015,
ISO 45001:2018.
Market: Scandinavian countries – Sweden, Norway, Denmark and Finland. The Swedish market is used
for modelling A4-A5 and C1-C4.
2.4 Technical Data
Technical Data – Hollow core slab
Name Value Unit
Compressive strength C40/50-C50/60 N/mm2
Reinforcing steel 7-Wire Strand, Y1860S7 Ø 9.3mm; -
12.5mm
Ultimate tensile strength (fpk) 1 860 N/mm2
Tensile 0,1 % proof-stress fp0,1k 1 580 N/mm2
Durability of product 50 years
Tolerances Svensk Betong "Toleranser för betongelement" 2020 Class А; B
Length: 1000 - 16000 mm, Width: 400 - 1200 mm, Height: 200-400 mm
2.5 HCS200; HCS220; HCS260; HCS320; HCS400 Base materials / Ancillary
Name Value Unit
Cement 15,7 m%
Aggregates 78,0 m%
Water 4,9 m%
Admixture 0,1 m%
Steel 1,4 m%
There is no biogenic carbon in the product.
2.6 Manufacturing
The manufacturing contains the following processes:
• Delivery of raw materials;
• Preparation of the metal molds, cutting and laying of the probation steel elements, placehold-
ers etc.;
Page | 3 AS BMGS - Precast concrete hollow core slab
• Concrete mixing and filling into the molds, curing;
• Removal of the formwork, finishing, storage.
Figure 1: Overview of the production route of precast concrete element (A1-A5, C1-C4, D)
2.7 Packaging
No packaging materials are used. The transportation does not cause any losses as products are secured
properly.
2.8 Production waste
The data on generated production waste is recorded as accurately as possible. Thus, the generated
production waste is allocated per declared unit. No loses for cement are assumed since filters are used
to collect dust in the air of cement storage in silos. The captured cement dust is reused in production.
No loses for inert materials are assumed too since materials are stored in open warehouses, which
three sides are enclosed by a wall. The same assumptions are made for other components. There is no
production waste for scrap metal, because reinforcement mesh, rebars and wires are delivered of the
size as in the drawings (no cutting is made).
Page | 4 AS BMGS - Precast concrete hollow core slab
3. LCA: Calculation rules
3.1 Declared unit
The EPD refers to the declared product system of 1 ton of precast concrete element.
Name Value Unit
Declared unit 1 ton
Cement type* СEM I 42.5R -
Compressive strength class** C40/50 - C50/60 -
Percentage of reinforcing steel 1,4 m%
7-Wire Strand, Y1860S7 -
Steel grade
Ø 9.3mm; 12.5mm
* СEM I 42.5R is used for LCA calculations. Starting from 2022 AS BMGS intends to use also CEM II A-M (S-LL) 52.5
N and CEM I 42,5 N SR3. Since the amount and the manufacturer of the cement used will not change it is expected
to have less environmental impact in some categories (e.g. GWP - “global warming potential”).
** Concrete mixes are produced according to recipes, in compliance with the strictest quality norms and stand-
ards in force, as well as the specific purposes for which a particular batch of concrete is intended.
3.2 System boundary
This EPD was created in accordance with EN 15804 requirements and include the production stage,
transportation to the site and construction, and the end-of-life stage. According to EN 15804 this cor-
responds to product phases A1-A5, C1-C4 and D (EPD type "Cradle to gate with options, modules C1-
C4 and module D" (A1-A3, C, D and additional modules A4 and A5)). All inputs including raw materials,
primary products, energy and auxiliary materials as well as the accumulated waste are considered in
the assessment. The use of the final product is not within the manufacturer's sphere of influence.
Therefore, modules B1-7 have not been considered. The effect of CO absorption through the carbon-
2
ization process is not taken into account in the LCA. The reference year is 2020. The geographical ref-
erence area is Latvia.
3.3 Estimates and assumptions
The raw material data for each of the product produced is recorded to a high standard of accuracy and
precision. The energy consumption, ancillary materials and production waste is allocated according to
the annual production of the declared unit to the total annual production at the factory (incl. averaging
the obtained data depending on the proportion of the total).
3.4 Cut-off criteria
All material flows that contribute to more than 1% of the total mass, energy or environmental impact
of the system have been considered in the LCA. It can be assumed that the neglected processes in total
contributed less than 5% to the considered impact categories.
The product stage includes materials, energy and waste flows only related to production processes
(e.g. energy and water use related to company management and sales activities are excluded where
technically possible; production, manufacture, and construction of manufacturing capital goods and
infrastructure, other processes which are not directly related to the production of concrete elements).
3.5 Background Data
The background data is taken from Ecoinvent database version 3.6. (2019). The life cycle assessment
was modeled with the Rethink tool. Geographical reference space of the background data is Latvia.
Almost all consistent datasets contained in the Ecoinvent database are documented and can be viewed
in the online Ecoinvent documentation.
Page | 5 AS BMGS - Precast concrete hollow core slab
3.6 Data quality
In the operating data survey, all relevant process-specific data had been collected. The data relating to
the manufacturing phase of the precast concrete element are determined by AS BMGS and refers to
production site in Riga, Tvaika iela 27. The data relating to the manufacturing construction phase are
determined also by BMGS and refers to the finished construction project in Sweden.
Secondary data were taken from the Ecoinvent 3.6 (2019) database. The database is regularly checked
and thus complies with the requirements of ISO 14040/44 (background data not older than 10 years).
The background data meets the requirements of EN 15804. The quantities of raw materials, consum-
ables and supplies used as well as the energy consumption have been recorded and averaged over the
entire year of operation.
The general rule has been that specific data from specific production processes or average data derived
from specific processes must be given priority when calculating an EPD or Life Cycle Assessment. Data
for processes that the manufacturer can not influence or choose, were backed up with generic data.
EPD of raw material (cement) was available but could not be integrated as it was calculated according
to EN 15804:2014 (+A1) and not according to the EN 15804:2020 (+A2) standard used here.
3.7 Period Under review
All process-specific data was collected for the operating year 2020. The quantities of raw and auxiliary
materials as well as energy consumption have been recorded and averaged over the entire operating
year 2020.
3.8 Allocation
There are no co-products in the raw material supply phase, so no allocation methods were used at this
stage. There are no allocations during the manufacturing phase at the plant.
3.9 Calculation methods
For life cycle assessment, the calculation methods described in ISO 14040 have been applied. The eval-
uation is based on the phases in the system boundaries.
3.10 Mix of electricity and CO -Certificates
2
The electricity mix was chosen according to the energy grid mix in Latvia (reference year 2019). No CO
2
certificates were counted.
3.11 Comparability
Basically, a comparison or an evaluation of EPD data is only possible if all the data sets to be compared
were created according to EN 15804 and the building context, respectively the product-specific char-
acteristics of performance, are considered.
3.12 Reference Service Life (RSL)
The concrete composition limits given in EN 206 are specified for an intended service life of at least 50
years under the respective exposure classes/ environmental conditions.
Page | 6 AS BMGS - Precast concrete hollow core slab
4. LCA: Scenarios and additional technical information
Module A4: This stage includes transport from the production stockyard to the construction site where
the prefabricated product shall be installed. Basic scenario transportation from AS BMGS production
sites in Latvia to customer in Sweden, Stockholm with distance radius around 100 km. Transportation
is calculated based on data form manufacturer and a scenario with the parameters described in the
following table. The transportation does not cause losses as products are secured properly.
Transport from production place to the construction site (A4)
Parameter Vehicle type Distance
Truck* Lorry >32t, EURO5 280 km**
Maritime Ferry/ Transoceanic freight ship, containers 270 km
* Data for transport is calculated for an average load factor, including empty return trips
** Total distance by truck: from Riga factory to the port located in Ventspils city (180 km) and from the port in
Sweden to the construction site (100 km)
Modules B1 to B7: For concrete components, maintenance and repair measures are generally not nec-
essary during the reference service life, so that no environmental burdens arise in these modules. In
addition, no energy or water is consumed.
C1 Demolition: According to the current state of the art, the demolition of concrete and reinforced
concrete structures is mainly carried out with longfront excavators equipped with demolition clamps.
The concrete buildings are demolished by so-called "press cutting", i.e. the crushing of concrete by
applying a compressive force. It is estimated that one site vehicle is in operation for 30 min per sqm of
concrete element (conservative assumption). In addition, based on Bozdağ, Ö & Seçer, M. (2007) en-
ergy consumption of a demolition process is on the average 10 kWh/m2 and an average mass of a
reinforced concrete building is about 1000 kg/m2. Therefore, energy consumption demolition is 10
kWh/1000 kg. The source of energy is diesel fuel used by work machines and based on the statements
above can be assumed being 1,009 l (with NCV 42,49 GJ/t).
C2 - C4 and D: It is assumed that concrete and reinforcement material are separated after deconstruc-
tion. For both waste groups, a waste scenario according to the Dutch National Environmental Database
(NMD) (SBK 2019) is applied:
• Concrete (i.a. elements, brickwork): 99% of concrete is recycled and reused as aggregate.
• Steel, reinforcement: 95% of reinforcing steel is marketed as scrap metal.
At the end-of-life, in the demolition phase 99% of steel and 90% concrete is assumed to be collected
as separate construction waste (C1). All of end-of-life product is assumed to be sent to the closest
facilities (C2).
The effect of CO2 absorption through the carbonization process in the use and end-of-life phase is not
assessed here and taken into account in the LCA.
Page | 7 AS BMGS - Precast concrete hollow core slab
5. LCA: Results
The following tables show the results of the impact assessment indicators, resource use, waste and
other output streams. The results presented here refer to the declared average product.
Description of the system boundary
Benefits and
Construction pro- loads beyond
Product stage Use stage End of life stage
cess stage the system
boundaries
y lp p u s la ir e t a m w a R t r o p s n a r T g n ir u t c a fu n a M u n a m m o r f t r o p s n a r T-e s u fo re ec ra ulp t c o at f n on io t cit ua rl tl sa nts on C-is s e c o r p e s U e c n a n e tn ia M r ia p e R tn e m e c a lp e R n e m h s ib r u fe Rt e s u y g r e n e la n o it a r e p O e s u r e t a w la n o it a r e p O -o m e d / n o it c u r ts n eo Dc -n o itil t r o p s n a r T g n is s e c o r p e ts a W la s o p s iD y r e v eo s uc ee RR -- gla ni it ln c ye ct o e Rp -
A1 A2 A3 A4 A5 B1 B2 B3 B4 B5 B6 B7 C1 C2 C3 C4 D
X X X X X MND MND MND MND MND MND MND X X X X X
X=Module declared | MND=Module not declared
Disclaimer on ADP-e, ADP-f, WDP, ETP-fw, HTP-c, HTP-nc, SQP: The results of these environmental
impact indicators must be used with caution, as the uncertainties in these results are high or as there
is limited experience with the indicator.
Disclaimer on IR: This impact category mainly addresses the potential effect of low dose ionizing radi-
ation on human health in the nuclear fuel cycle. It does not consider effects due to possible nuclear
accidents and occupational exposures, nor does it consider radioactive waste disposal in underground
facilities. Potential ionizing radiation from soil, radon, and some building materials is also not measured
by this indicator.
Page | 8 AS BMGS - Precast concrete hollow core slab
Results of the LCA – Environmental impact: 1 t of precast concrete hollow core slab
Parameter Unit A1 A2 A3 A4 A5 C1 C2 C3 C4 D
Core environmental impact indicators (EN 15804)
ADP-mm kg Sb-eqv. 1,68E-03 2,20E-04 3,80E-05 4,31E-04 3,19E-03 5,07E-06 1,64E-04 4,48E-06 5,08E-07 -2,04E-04
ADP-f MJ 8,03E+02 1,31E+02 2,14E+02 4,07E+02 5,55E+02 4,55E+01 9,78E+01 2,13E+01 1,55E+00 -5,11E+01
AP mol H+ eqv. 4,24E-01 5,04E-02 3,00E-02 1,80E-01 2,81E-01 3,46E-02 3,76E-02 9,97E-03 5,27E-04 -2,96E-02
EP-fw kg P eqv. 3,11E-03 8,77E-05 7,31E-05 1,94E-04 1,70E-03 1,20E-05 6,54E-05 4,95E-05 6,23E-07 -1,51E-04
EP-m kg N eqv. 1,05E-01 1,78E-02 7,83E-03 4,99E-02 8,58E-02 1,53E-02 1,33E-02 3,97E-03 1,81E-04 -8,47E-03
EP-T mol N eqv. 1,34E+03 1,17E+02 5,48E+01 3,20E+02 1,05E+03 2,74E+01 8,72E+01 1,73E+01 1,01E+00 -8,24E+01
GWP-b kg CO2 eqv. 2,39E+00 4,01E-03 1,08E-01 1,68E-02 3,86E-01 9,20E-04 2,99E-03 9,19E-03 1,10E-04 -1,89E-02
GWP-f kg CO2 eqv. 1,55E+02 8,69E+00 1,48E+01 2,66E+01 6,13E+01 3,31E+00 6,48E+00 1,59E+00 5,55E-02 -4,10E+00
GWP-luluc kg CO2 eqv. 1,63E-01 3,19E-03 2,80E-03 8,74E-03 1,10E-01 2,61E-04 2,38E-03 3,02E-04 1,55E-05 -4,40E-03
GWP-total kg CO2 eqv. 1,58E+02 8,70E+00 1,49E+01 2,66E+01 6,18E+01 3,31E+00 6,49E+00 1,60E+00 5,57E-02 -4,12E+00
ODP kg CFC 11 eqv. 6,17E-06 1,92E-06 2,05E-06 6,17E-06 5,22E-06 7,14E-07 1,43E-06 2,06E-07 2,29E-08 -4,09E-07
POCP kg NMVOC eqv. 3,23E-01 5,59E-02 2,99E-02 1,64E-01 2,67E-01 4,61E-02 4,17E-02 1,20E-02 5,81E-04 -2,72E-02
WDP m3 world eqv. 2,78E+01 4,69E-01 -2,36E-01 1,27E+00 1,65E+01 6,10E-02 3,50E-01 9,67E-02 6,96E-02 -5,88E+01
Additional environmental impact indicators (EN 15804)
ETP-fw CTUe 1,22E+00 1,96E-01 8,62E-02 5,53E-01 9,55E-01 1,68E-01 1,46E-01 4,41E-02 2,00E-03 -9,83E-02
HTP-c CTUh 1,82E-07 3,79E-09 3,42E-09 8,76E-09 1,23E-07 9,59E-10 2,83E-09 4,10E-10 2,33E-11 -3,05E-09
HTP-nc CTUh 5,53E-06 1,28E-07 4,34E-08 3,57E-07 3,50E-06 2,36E-08 9,54E-08 1,16E-08 7,16E-10 -8,61E-08
IR kBq U235 eqv. 3,59E+00 5,49E-01 3,02E-01 1,78E+00 2,04E+00 1,95E-01 4,10E-01 6,76E-02 6,37E-03 -2,06E-01
PM disease incidence 3,63E-06 7,82E-07 2,85E-07 2,26E-06 4,32E-06 9,17E-07 5,83E-07 2,20E-07 1,02E-08 -5,10E-07
SQP Pt 2,75E+02 1,14E+02 2,79E+01 4,35E+02 4,57E+02 5,81E+00 8,48E+01 3,56E+00 3,26E+00 -6,60E+01
ADP-e=Depletion of abiotic resources-elements | ADP-f=Depletion of abiotic resources-fossil fuels | AP=Acidification of soil and water | EP-fw =Eutrophication, freshwater | EP-m=Eutrophication marine | EP-T=Eutrophi-
cation, terrestrial | GWP-b=Global warming potential - Biogenic | GWP-f=Global warming potential - Fossil | GWP-luluc=Global warming potential - Land use and land use change |GWP-total=Global warming potential
|ODP=Ozone layer depletion |POCP=Photochemical oxidants creation | WDP=Water use | ETP-fw=Ecotoxicity, freshwater | HTP-c=Human toxicity, cancer | HTP-nc=Human toxicity, non-cancer | IR=Ionising radiation,
human health | PM=Particulate Matter | SQP=Land use
Page | 9 AS BMGS - Precast concrete hollow core slab
Resource use and environmental information: 1 t of precast concrete hollow core slab
Parame-
Unit A1 A2 A3 A4 A5 C1 C2 C3 C4 D
ter
PERE MJ 6,23E+01 1,64E+00 9,42E+00 4,95E+00 2,76E+01 2,46E-01 1,22E+00 1,21E+00 1,26E-02 -3,54E+00
PERM MJ 0,00E+00 0,00E+00 0,00E+00 0,00E+00 0,00E+00 0,00E+00 0,00E+00 0,00E+00 0,00E+00 0,00E+00
PERT MJ 6,23E+01 1,64E+00 9,42E+00 4,95E+00 2,76E+01 2,46E-01 1,22E+00 1,21E+00 1,26E-02 -3,54E+00
PENRE MJ 8,52E+02 1,39E+02 2,33E+02 4,32E+02 5,91E+02 4,83E+01 1,04E+02 2,27E+01 1,65E+00 -5,43E+01
PENRM MJ 0,00E+00 0,00E+00 2,13E+00 0,00E+00 0,00E+00 0,00E+00 0,00E+00 0,00E+00 0,00E+00 0,00E+00
PENRT MJ 8,52E+02 1,39E+02 2,36E+02 4,32E+02 5,91E+02 4,83E+01 1,04E+02 2,27E+01 1,65E+00 -5,43E+01
SM Kg 1,37E+01 0,00E+00 0,00E+00 0,00E+00 9,29E+00 0,00E+00 0,00E+00 0,00E+00 0,00E+00 0,00E+00
RSF MJ 0,00E+00 0,00E+00 0,00E+00 0,00E+00 0,00E+00 0,00E+00 0,00E+00 0,00E+00 0,00E+00 0,00E+00
NRSF MJ 0,00E+00 0,00E+00 0,00E+00 0,00E+00 0,00E+00 0,00E+00 0,00E+00 0,00E+00 0,00E+00 0,00E+00
FW m3 1,38E+00 1,60E-02 8,79E-03 4,45E-02 5,21E-01 2,34E-03 1,19E-02 7,13E-03 1,66E-03 -1,38E+00
HWD Kg 9,55E-04 3,32E-04 2,84E-04 9,41E-04 1,34E-03 1,24E-04 2,48E-04 3,72E-05 2,32E-06 -1,03E-04
NHWD Kg 7,57E+00 8,32E+00 5,36E-01 3,28E+01 2,08E+01 5,39E-02 6,20E+00 2,97E+00 1,05E+01 -5,54E-01
RWD Kg 3,71E-03 8,61E-04 3,79E-04 2,78E-03 2,48E-03 3,16E-04 6,42E-04 9,58E-05 1,02E-05 -2,24E-04
CRU Kg 0,00E+00 0,00E+00 0,00E+00 0,00E+00 0,00E+00 0,00E+00 0,00E+00 0,00E+00 0,00E+00 0,00E+00
MFR Kg 0,00E+00 0,00E+00 1,27E+01 0,00E+00 8,83E+00 0,00E+00 0,00E+00 9,89E+02 0,00E+00 0,00E+00
MER Kg 0,00E+00 0,00E+00 0,00E+00 0,00E+00 0,00E+00 0,00E+00 0,00E+00 0,00E+00 0,00E+00 0,00E+00
EE MJ 0,00E+00 0,00E+00 1,04E+00 0,00E+00 0,00E+00 0,00E+00 0,00E+00 0,00E+00 0,00E+00 0,00E+00
EET MJ 0,00E+00 0,00E+00 6,60E-01 0,00E+00 0,00E+00 0,00E+00 0,00E+00 0,00E+00 0,00E+00 0,00E+00
EEE MJ 6,23E+01 1,64E+00 9,42E+00 4,95E+00 2,76E+01 2,46E-01 1,22E+00 1,21E+00 1,26E-02 -3,54E+00
PERE=renewable primary energy ex. raw materials | PERM=renewable primary energy used as raw materials | PERT=renewable primary energy total | PENRE=non-renewable primary energy ex. raw materials |
PENRM=non-renewable primary energy used as raw materials | PENRT=non-renewable primary energy total | SM=use of secondary material | RSF=use of renewable secondary fuels | NRSF=use of non-renewable
secondary fuels | FW=use of net fresh water | HWD=hazardous waste disposed | NHWD=non-hazardous waste disposed | RWD=radioactive waste disposed | CRU=Components for re-use | MFR=Materials for recycling |
MER=Materials for energy recovery | EE=Exported energy | EET=Exported Energy Thermic | EEE=Exported Energy Electric
Page | 10 AS BMGS - Precast concrete hollow core slab
6. LCA: Interpretation
The following figure shows the influence of the different life stages on the environmental core indica-
tors for precast concrete massive slab. Since the Global Warming Potential biogen (GWP-b) and Global
Warming Potential resulting from land use and land use (GWP-luluc) change have only a minor impact,
only total Global Warming Potential (GWP-total) is displayed. As shown in Figure 1 the majority of the
environmental impact is attributed to row material processing phase (A1), followed by the transports
of raw materials (A2) and production (A3). Results of processing phase (A1) theoretically can be ex-
pected lower since the supplier of the main raw material – cement, is implementing environmental
policy, for example, for cement manufacturing process different alternatives to fossil fuels are used,
as used tires, tire fluffy, NPS: Neutralized Polluted Soil (NPS) and Solid Recovered Fuel (SRF). In addi-
tion, this supplier owns the “Powered by green” certificate which confirms that the company is buying
electricity produced in Latvia from 100% renewable energy sources. But EPD of cement could not be
used because it is still calculated according to the old standard (EN 15804+A1), therefore secondary
data had to be used.
Hollow core slabs
100%
80%
60%
40%
20%
0%
-20%
-40%
-60%
-80%
-100%
A1 A2 A3 A4 A5 C1 C2 C3 C4 D
Figure 2: Influence of the modules on the environmental core indicators
Overall, the quality of the data can be considered as good. The primary data collection has been done
thoroughly. Data quality was calculated using the Data Quality Rating method according to the PEF
approach. The DQRs range from 1,67 to 2,33 for the most abundant inputs in terms of mass.
Page | 11 AS BMGS - Precast concrete hollow core slab
7. Additional information: Norwegian requirements
Greenhouse gas emissions from the use of electricity mix in the manufacturing phase
Data source Amount Unit
Ecoinvent 3.6 (year 2019) 0,146 CO2-eqv/kWh
Dangerous substances disclaimer
The product contains no substances given by the REACH Candidate list or the Norwegian pri-
☒
ority list
The product contains substances given by the REACH Candidate list or the Norwegian priority
☐
list that are less than 0,1 % by weight.
The product contain dangerous substances, more then 0,1% by weight, given by the REACH
☐
Candidate List or the Norwegian Priority list, see table.
The product contains no substances given by the REACH Candidate list or the Norwegian pri-
☐
ority list. The product is classified as hazardous waste (Avfallsforskiften, Annex III), see table.
Indoor environment
The product has not been tested for emissions to indoor environment. The product contains no dan-
gerous substances on the REACH Candidate list or the Norwegian priority list, and a water-based re-
lease agent is used. Based on this it is assumed that the product has a negligible impact on the indoor
environment.
Carbon footprint
Carbon footprint has not been worked out for the product.
Page | 12 AS BMGS - Precast concrete hollow core slab
8. References
Augstsprieguma tikls (AST) - Latvian electricity market overview: https://www.ast.lv/en/electricity-
market-review?year=2020&month=13; accessed 27th of January 2022
Bozdağ, Ö., Seçer, M. (2007) - Energy consumption of demolition process is on the average
CML-IA April 2013 – Characterisation factors developed by Institute of Environmental Sciences (CML):
University Leiden (NL)- http://www.cml.leiden.edu/software/data-cmlia.html
European Commission Joint Research Centre Institute for Prospective Technological Studies (JCR
2014): End-of-waste criteria for waste plastic for conversion, Seville, 2014, doi:10.2791/13033
Liebherr’s Rental - https://www.liebherr-rental.co.uk/; accessed 29th of January 2022
SCHWENK Latvija, SIA (2019) Environmental Product Declaration CEM I 42.5 R, CEM II A-M (S-LL) 52.5
N, CEM I 42.5 N SR-3
Stichting Bouwkwaliteit (SBK 2019): Assessment Method - Environmental Performance Construction
and Civil Engineering Works (GWW), Rijswijk, Version "3.0 January 2019" incl. amendments July 2019,
Jan 2020
Stichting Bouwkwaliteit: verification protocol - inclusion data in the Dutch environmental database,
Rijswijk, Final Version 3.0, January 2019
REACH Regulation (EC) No 1907/2006 of the European Parliament and of the Council on the Registra-
tion, Evaluation, Authorisation and Restriction of Chemicals (REACH) https://echa.europa.eu/candi-
date-list-table; accessed 27th of January 2022, 223 substances listed
Standards and laws
ISO 14040:2006-10, Environmental management - Life cycle assessment - Principles and framework;
EN ISO 14040:2006
ISO 14044:2006, Environmental management - Life cycle assessment - Requirements and guidelines;
EN ISO 14040:2006
ISO 14025:2011-10, Environmental labels and declarations - Type III environmental declarations - Prin-
ciples and procedures EN 13249
EN 15804:2014 (+A1), Sustainability of construction works - Environmental Product Declarations - Core
rules for the product category of construction products
EN 15804:2020 (+A2) Sustainability of construction works - Environmental product declarations - Core
rules for ,the product category of construction products
EN 16757:2017, Sustainability of construction works - Environmental product declarations -Product
Category Rules for concrete and concrete elements
ISO 21930:2007, Sustainability in building construction - Environmental declaration of building prod-
ucts
Page | 13 AS BMGS - Precast concrete hollow core slab
Publisher Mail DE.Ecobility.Ex-
Kiwa - Ecobility Experts perts@kiwa.com
Kiwa GmbH Web https://www.kiwa.com/de/de
Voltastr.5, 13355 Berlin /uber-kiwa/ecobility-experts/
Germany
Programme operator Mail DE.Ecobility.Ex-
Kiwa - Ecobility Experts perts@kiwa.com
Kiwa GmbH Web https://www.kiwa.com/de/de
Voltastr.5, 13355 Berlin /uber-kiwa/ecobility-experts/
Germany
Author of the Life Cycle Tel. +49 (0)30 467761-43
Assessment Fax. +49 (0)30 467761-10
Kiwa GmbH Mail martin.koehrer@kiwa.de
Voltastr.5, 13355 Berlin Web https://www.kiwa.com/
Germany
Inspecta Latvia AS Tel. +371 67 607 900
Skanstes iela 54a Fax. +371 67 607 901
LV-1013 Riga, Mail jekaterina.krastina@kiwa.com
Latvia Web https://www.kiwa.com/lv
Owner of the declaration Tel. +371 67 272 717
BMGS AS Mail info@bmgs.lv
Tvaika iela 27 Web https://www.bmgs.lv
LV-1005 Riga
Latvia
Page | 14 AS BMGS - Precast concrete hollow core slab
