ENVIRONMENTAL PRODUCT DECLARATION
as per ISO 14025 and EN 15804+A2
Owner of the Declaration VELUX Group
Publisher Institut Bauen und Umwelt e.V. (IBU)
Programme holder Institut Bauen und Umwelt e.V. (IBU)
Declaration number EPD-VEL-20230280-IBA2-EN
Issue date 21.08.2023
Valid to 20.08.2028
VELUX sun tunnel TLF for pitched roof, flexible
VELUX A/S
www.ibu-epd.com | https://epd-online.com
1. General Information
VELUX A/S VELUX sun tunnel TLF for pitched roof, flexible
Programme holder Owner of the declaration
IBU – Institut Bauen und Umwelt e.V. VELUX Group
Hegelplatz 1 Ådalsvej 99
10117 Berlin 2970 Hørsholm
Germany Denmark
Declaration number Declared product / declared unit
EPD-VEL-20230280-IBA2-EN The declaration represents 1 piece of VELUX sun tunnel TLF for pitched
roof, flexible.
This declaration is based on the product category rules: Scope:
Windows and doors , 01.08.2021 The declaration covers 100% of VELUX sun tunnel TLF for pitched roof,
(PCR checked and approved by the SVR) flexible by Partizánske Building Components SK, Slovakia.
The owner of the declaration shall be liable for the underlying information
Issue date and evidence; the IBU shall not be liable with respect to manufacturer
information, life cycle assessment data and evidences.
21.08.2023
The EPD was created according to the specifications of EN 15804+A2. In
the following, the standard will be simplified as EN 15804.
Valid to
20.08.2028 Verification
The standard EN 15804 serves as the core PCR
Independent verification of the declaration and data according to ISO
14025:2011
internally X externally
Dipl.-Ing. Hans Peters
(Chairman of Institut Bauen und Umwelt e.V.)
Florian Pronold Dr. Matthew Fishwick,
(Managing Director Institut Bauen und Umwelt e.V.) (Independent verifier)
1 Environmental Product Declaration - VELUX A/S - VELUX sun tunnel TLF for pitched roof, flexible
2. Product
Acrylic adhesive 2%
2.1 Product description/Product definition Glass 27%
Flexible sun tunnel TLF is used for installation in pitched roofs Steel 1%
and flat roofing materials which brings natural light into areas of Others 5%
the house where a VELUX roof window installation is either not
possible or not appropriate. The dark grey frame with integrated 1) 'This product/article/at least one partial article contains
flashing is made of lacquered aluminium. Sash and diffuser unit substances listed in the ECHA candidate list (date: 02.03.2022)
are made of plastic. The tunnel is made of flexible reflective exceeding 0.1 percentage by mass:
material.
• no
2) 'This product/article/at least one partial article contains other
For the placing of the product on the market in the European
carcinogenic, mutagenic, or toxic for reproduction (CMR)
Union/European Free Trade Association (EU/EFTA) (with the
substances in categories 1A or 1B which are not on the ECHA
exception of Switzerland) the Regulation (EU) No. 305/2011/
candidate list, exceeding 0.1 percentage by mass:
(CPR) applies. The product needs a declaration of performance
in accordance with the CPR taking into the European Technical • not investigated with suppliers
Assessment: ETA -13/0764 of 14/10/2015. The CE-marking for 3) 'Biocide products were added to this construction product or
the product takes into account the Declaration of Performance it has been treated with biocide products (this then concerns a
in accordance with the CPR. For the application and use the treated product as defined by the (EU) Regulation on Biocidal
respective national provisions apply. Products No. 528/2012):
• no
2.2 Application
The sun tunnel for pitched roofs can be installed in roof pitches
between 15° and 60°. The sun tunnel can be integrated in flat
Recycled content
roofing materials like roofing felt or slates/shingles.
2.3 Technical Data
The Declaration of Performance including relevant technical
specifications and test methods/test standards can be
downloaded from the website www.velux.com/ce.
Constructional data for TLF 0K14 2010
For other variants, see velux.com/ce
Name Value Unit
The values stated in the table relate to the recycled material
Reaction to fire E class
streams in VELUX production.
Resistance to upward load EN 1875 C3 -
Resistance to downward load EN 1873 C3 - 2.6 Manufacture
A few components are produced/processed internally. The
Resistance to fire EN 13501-2 NPD -
majority of products are bought from external suppliers and
External fire performance EN 13501-5 NPD -
assembled into the final product.
Water tightness EN 1873 9A -
Impact resistance - small hard body passed The factory is ISO 9001 certified.
NPD -
EN 1873
2.7 Environment and health during manufacturing
Impact resistance - large soft body EN 1873 NPD -
The factory is ISO14001 and ISO 45001 certified.
Direct airborne sound insulation EN ISO 54 (-5;-
dB
410-3 9)
2.8 Product processing/Installation
Thermal transmittance EN 1873 2.5 W/(m2K) The sun tunnel is fitted directly to the roof with the screws
Luminous transmittance EN 410 NPD - supplied.
Air permeability EN 1026 4 Class It is important that frame and roofing material are fitted
according to the installation instructions. Distance from interior
Durability EN 1873 passed -
ceiling finish to the upper edge of battens (measured in the
Performance data of the product in accordance with the centre of the tunnel): 0.2 - 0.9 m
declaration of performance with respect to its essential Installation of a sun tunnel requires access to the attic and the
characteristics according to ETA -13/0764 of 14/10/2015. roof.
Performance data of the product, based on the harmonised
standards, in accordance with the other provisions for 2.9 Packaging
harmonization. The packaging usually consists of:
- cardboard
2.4 Delivery status
- paper
The product is available in a diameter of 350 mm. - polyethylene film
- polystyrene foam parts
2.5 Base materials/Ancillary materials
- steel
Composition of the sun tunnel TLF 0K14 2010:
Acrylonitrile Butadiene Styrene (ABS) 16%
The use of other packaging materials is possible, but
Polycarbonate 13%
insignificant in terms of quantity.
Polyethylene 3%
Stainless steel 10%
The plastic packaging (polyethylene (PE) film, polystyrene foam
Aluminium 23%
2 Environmental Product Declaration - VELUX A/S - VELUX sun tunnel TLF for pitched roof, flexible
parts), paper and cardboard as well as steel can be recycled if
separated by type; alternatively, they - except steel - can be Water
incinerated. In the event of unforeseen exposure to water (flood), no
adverse effects on human health or the environment are to be
2.10 Condition of use expected.
The material composition of VELUX sun tunnels does not
change over their service life. Mechanical destruction
In the event of unforeseen mechanical destruction, VELUX sun
2.11 Environment and health during use
tunnels have to be replaced; apart from potential injuries from
VELUX sun tunnels do not contain any pollutants that could be sharp edges, no adverse effects on human health or the
released during use. environment are to be expected.
Environmental protection: According to current knowledge, 2.14 Re-use phase
hazards to water, air and soil cannot arise when the products VELUX sun tunnels can be dismantled manually without any
are used as intended. problems. The metal parts are usually recycled, and the plastic
parts are sent for thermal recycling for energy recovery.
Health protection: According to current knowledge, no health Tempered glass can be recycled.
hazards or impairments are to be expected.
2.15 Disposal
2.12 Reference service life VELUX sun tunnels are mostly inert and can be disposed of in
It is not possible to calculate the reference service life an appropriate landfill. However, due to the value of the
according to ISO 15686. The service life based on a materials or the carbon content of the plastic parts, recycling or
manufacturer's declaration is 30 years. The corresponding energy recovery is preferable and common.
utilization scenario is declared in 4.
Waste code according to the European Waste List (Regulation
2.13 Extraordinary effects
on the European Waste List):
Fire 17 02 02 glass
Fire performance according to EN 13501-1 17 02 03 plastics
17 04 14 mixed metals
Name Value
Building material class B 2.16 Further information
Burning droplets s1 Further documentation on the products, technical data sheets,
Smoke gas development d0 BIM files, etc. can be found at:
www.velux.com
3. LCA: Calculation rules
municipal waste incineration plant with an efficiency R1 < 0.6
3.1 Declared Unit (according to the ecoinvent v3.8 (cut-off) dataset used); the
The declared unit is 1 piece of VELUX sun tunnel TLF for recovered energy is declared as exported energy. Metals,
piched roof, flexible (TLF 0K14 2010) for a diameter of 350 mm. paper and cardboard are recycled; it is assumed that these
Declared unit fractions reach the end-of-waste state after having been sorted
and transported (as a conservative choice) to a recycler. No
Name Value Unit
packaging waste is landfilled.
Declared unit 1 piece
Area 0.1225 m² Modules B1 to B7 are not relevant for the product under
Mass reference 6.19 kg/pce consideration or no significant environmental impacts occur.
Module C1 includes manual dismantling, with no significant
3.2 System boundary environmental impact.
Type of EPD: Cradle to gate with options, with modules C1 –
Module C2 comprises the transport of the dismantled VELUX
C4, and module D (A1-A3, C, D and additional modules)
sun tunnel to a sorting plant and then to a waste incineration
plant for the thermally treated plastic fraction.
The production of VELUX sun tunnels (modules A1-A3)
includes raw material extraction, energy generation, waste
Modules C3/C4: given the complexity of the inventoried
treatment and all transports up to the factory gate. In
products, a mixed end-of-life scenario is modelled, allowing the
accordance with COUNCIL REGULATION (EU) No 333/2011,
different materials to follow their most likely path.
secondary metals are modelled as part of the product system
As a rule of thumb, metals are recycled and plastics are
from the moment they are available as unmixed scrap.
incinerated (also due to the very limited data available on
Waste or secondary fuels are not used for production.
plastics recycling and its benefits); tempered glass is assumed
to be recycled; it is assumed that these fractions reach the end-
Module A4 is not declared due to large variances in transport
of-waste state after having been sorted and transported to a
distances between the production site and the construction site,
recycler. The combustible material (plastics, etc.) is assumed to
where the product is installed.
be thermally treated in a municipal waste incineration plant.
Module A5: The products are delivered to the construction site
Module D includes the benefits and burdens associated with
ready to be installed. Manual installation is assumed; electricity
recycling metals beyond the system boundary, resulting from
consumption related to electric drilling machines, screwdrivers,
the treatment of recycled materials from the point of end-of-
etc. is considered to be negligible. The combustible packaging
waste to the point of substitution (as loads) and substitution of
material (plastics) is assumed to be thermally treated in a
3 Environmental Product Declaration - VELUX A/S - VELUX sun tunnel TLF for pitched roof, flexible
primary resources (as benefits).
It also includes the benefits and burdens associated with 3.7 Period under review
energy recovery from plastic waste in a municipal waste The LCA data represents the production conditions for the year
incineration plant, as modelled in Module C3. 2021.
In Module D, only net flows of metals leaving the product
3.8 Geographic Representativeness
system are considered.
Land or region, in which the declared product system is
3.3 Estimates and assumptions manufactured, used or handled at the end of the product´s
No further assumptions and estimates relevant to the result had lifespan: Europe
to be made beyond the points made in this chapter 3 and
chapter 4.
3.9 Allocation
No co-products are generated during the production of the
3.4 Cut-off criteria VELUX products. Sorted production scrap of the different
No data available from the company survey was neglected. metals, notably aluminium, is considered a secondary material
These include, among other things, material use, energy with no economic value (so no burdens allocated) and
demand (heat, electricity), packaging materials of raw materials considered in the quantification of net flows leaving the product
(in so far as they are generated as waste) and product system. This approach is chosen to ensure a coherent
packaging, consumables in production, waste treatment and quantification of net flows entering module D.
the transport of all inputs and outputs.
With this approach, mass and energy flows below 1% were also No processes were modelled as part of the foreground model
accounted for, up to a total of 5%. No processes were that would have required an allocation of multi-input processes.
neglected that would have been known to the project managers Background datasets on municipal waste incineration plants
and would have contributed significantly to the indicators of the were taken from ecoinvent v3.8 (cut-off) without any
impact assessment. modification.
3.5 Background data Allocation of reuse, recycling and recovery was avoided by the
Ecoinvent v3.8 (cut-off) (2021) is used as the background cut-off approach in the foreground model in line with DIN EN
database. 15804.
3.6 Data quality 3.10 Comparability
The foreground data are based on extensive and detailed data Basically, a comparison or an evaluation of EPD data is only
collection at the production site. The foreground data could be possible if all the data sets to be compared were created
fully linked with corresponding data records from the according to EN 15804 and the building context, respectively
background database ecoinvent v3.8 (cut-off). the product-specific characteristics of performance, are taken
The background data was updated in 2021. Thus, the quality of into account.
the foreground and background data can be rated as very Ecoinvent v3.8 (cut-off) has been used as the background
good. database.
4. LCA: Scenarios and additional technical information
and transported (as a conservative choice) to a recycler over
Characteristic product properties of biogenic carbon 150 km with a lorry with a payload of 16-32 metric tons,
Information on describing the biogenic carbon content at EURO6.
factory gate No packaging waste is landfilled.
The use of multi-way pallets is not taken into account as
Name ValueUnit
packaging material.
kg
Biogenic carbon content in product -
C
Biogenic carbon content in accompanying kg
< 5%
packaging C
Note: 1 kg of biogenic carbon is equivalent to 44/12 kg of CO .
2
Module A5
The products are delivered to the construction site ready to be
installed. Manual installation is assumed, and electricity
consumption related to electric drilling machines, screwdrivers,
etc. is considered to be negligible.
The combustible packaging material (plastics) is assumed to be
transported 50 km with a lorry with a payload of 16-32 metric
tons, EURO6 to an incineration plant with an efficiency R1 < 0.6
(according to the ecoinvent v3.8 (cut-off) dataset used); the
recovered energy is declared as exported energy; for its
quantification, an efficiency of 25.6% is assumed for the
production of heat and 13.0% for the production of electricity
(always referring to the lower heating value of the waste).
Metals and cardboard are recycled; it is assumed that these
fractions reach the end-of-waste state after having been sorted
4 Environmental Product Declaration - VELUX A/S - VELUX sun tunnel TLF for pitched roof, flexible
Module C2
Given the complexity of the inventoried products, a mixed end-
of-life scenario is modelled, allowing the different materials to
follow their most likely path.
It should also be noted that the deconstruction and waste
treatment scenario can vary a lot, depending on the actual
situation. Thus, a generic end-of-life scenario is assumed.
As a rule of thumb, metals are recycled, plastics are incinerated
(also due to the very limited availability on plastics recycling
and its benefits); coated and uncoated flat glass is assumed to
be recycled whereas laminated glass is assumed to be
landfilled due to very limited recycling
Reference service life potential.
Name Value Unit The combustible material (mainly plastics) is assumed to be
transported 50 km with a lorry 16-32 metric tons, EURO6 to an
Reference service life
incineration plant.
according to 30 a
Metals and tempered glass aredrecycled; it is assumed that
manufacturer's declaration
these fractions reach the end-of-waste state after having been
The product has passed
Declared product sorted and transported to a recycler over 150 km with a lorry
internal quality controls and
properties (at the gate) and - 16-32 metric tons, EURO6.
complies with EN 1873 for CE
finishes
marking
Module C3
An assumed quality of A consumption of 0.03 kWh/kg of electricity for shredding and
Carried out in accordance
work, when installed in sorting and 0.437 MJ/kg of diesel fuel for internal logistics are
with the manufacturer's -
accordance with the taken into account to disassemble the product. The recovered
instructions.
manufacturer’s instructions material leaves the product system as 'materials for recycling'.
Design application The net amounts of the metals leaving the product system are
parameters (if instructed by considered as 'use of secondary material' in Module D.
Installation according to
the manufacturer),
assembly instructions and -
including the references to Module C4
state of the art.
the appropriate practices As stated above, it is assumed that 100% of the plastic parts
and application codes are treated in a waste incineration plant with an efficiency R1
Outdoor environment, (for The declared products are < 0.6 (according to the ecoinvent v3.8 (cut-off) dataset used);
outdoor applications), e.g. intended for installation 25.57% of the lower heating value of the plastic parts are
weathering, pollutants, UV outside the building: They are recovered as heat and 13.0% as electricity. Recovered energy
and wind exposure, therefore designed to - is reported as 'exported energy' and considered in Module D.
building orientation, withstand outdoor conditions
shading, temperature throughout their service life. Module D
Module D contains the benefits and loads beyond the system
Indoor environment (for
The declared products are boundary related to the recycling of metals, which result from
indoor applications), e.g.
not intended for installation - the treatment of recycled materials from the point of end-of-
temperature, moisture,
inside a building. waste status to the point of substitution (as loads) and the
chemical exposure
substitution of primary resources (as benefits).
Usage conditions, e.g. Standard use in any type of
Furthermore, it includes the benefits of raw material substitution
frequency of use, building, i.e. opening/closing -
of the recycling of tempered glass. Recovered tempered glass
mechanical exposure as often as necessary.
is assumed to have reached the end-of-waste state as sorted
The declared products are glass cullet; glass cullet is assumed to replace virgin raw
Maintenance e.g. required designed for a reference life material for glass production – impacts on the energy required
frequency, type and quality of 30 years. They are - to remelt recycled glass as compared to virgin glass production
and replacement of maintained by cleaning water are neglected due to a lack of data.
components at the discretion of the It also includes the benefits and loads related to the energy
building occupants. recovery from plastic wastes in a MWIP as modelled in
Modules A3, A5 and C3.
Module C1 Due to a lack of data for plastics from de-construction activities,
Manual de-installation is assumed, electricity consumption the substitution potential of recycled plastics is not taken into
related to electric screw drivers, etc. is considered to be account.
negligible. Thus, no environmental impacts are declared in Only net flows leaving the product system are considered in
module C1. module D.
5 Environmental Product Declaration - VELUX A/S - VELUX sun tunnel TLF for pitched roof, flexible
5. LCA: Results
DESCRIPTION OF THE SYSTEM BOUNDARY (X = INCLUDED IN LCA; MND = MODULE OR INDICATOR NOT DECLARED; MNR
= MODULE NOT RELEVANT)
Benefits and
Construction loads beyond
Product stage Use stage End of life stage
process stage the system
boundaries
la ire ta m w a Ry lp p u s tro p s n a rT g n iru tc a fu n a M e h t m o rf tro p s n a rTe tis e h t o t e ta g y lb m e s s A e s U e c n a n e tn ia M ria p e R tn e m e c a lp e R tn e m h s ib ru fe R y g re n e la n o ita re p Oe s u re ta w la n o ita re p Oe s u n o itc u rts n o c -e Dn o itilo m e d tro p s n a rT g n is s e c o rp e ts a W la s o p s iD -e s u e R-y re v o c e R-g n ilc y c e Rla itn e to p
A1 A2 A3 A4 A5 B1 B2 B3 B4 B5 B6 B7 C1 C2 C3 C4 D
X X X MND X MND MND MNR MNR MNR MND MND X X X X X
RESULTS OF THE LCA - ENVIRONMENTAL IMPACT according to EN 15804+A2: 1 piece VELUX sun tunnel TLF 0K14 2010 for
pitched roof, flexible
Parameter Unit A1-A3 A5 C1 C2 C3 C4 D
GWP-total kg CO 2 eq 4.96E+01 4.15E+00 0 6.39E-02 1.99E-01 5.7E+00 -2.95E+01
GWP-fossil kg CO 2 eq 5.34E+01 2.52E-01 0 6.39E-02 1.39E-01 5.7E+00 -2.94E+01
GWP-biogenic kg CO 2 eq -3.96E+00 3.9E+00 0 0 5.91E-02 0 0
GWP-luluc kg CO 2 eq 1.33E-01 4.33E-05 0 2.6E-05 1.55E-04 9.97E-05 -9.61E-02
ODP kg CFC11 eq 2.76E-06 2.49E-08 0 1.5E-08 8.58E-09 3.72E-08 -1.13E-06
AP mol H+ eq 2.81E-01 6.15E-04 0 3.62E-04 5.32E-04 1.46E-03 -1.75E-01
EP-freshwater kg P eq 1.67E-03 7.9E-07 0 4.7E-07 1.81E-05 3.13E-06 -1.23E-03
EP-marine kg N eq 5.14E-02 2.23E-04 0 1.3E-04 1.71E-04 6.17E-04 -2.62E-02
EP-terrestrial mol N eq 5.36E-01 2.46E-03 0 1.43E-03 1.94E-03 6.66E-03 -2.92E-01
kg NMVOC
POCP 1.76E-01 7E-04 0 4.1E-04 5.17E-04 1.7E-03 -8.69E-02
eq
ADPE kg Sb eq 1.4E+01 3.57E-07 0 2.14E-07 2.43E-07 8.29E-07 1.7E-04
ADPF MJ 6.36E+02 1.63E+00 0 9.84E-01 1.92E+00 1.25E+00 -2.85E+02
m3 world eq
WDP 1.4E+01 5.57E-03 0 3.23E-03 4.79E-03 6.24E-02 -3.9E+00
deprived
GWP = Global warming potential; ODP = Depletion potential of the stratospheric ozone layer; AP = Acidification potential of land and water; EP =
Eutrophication potential; POCP = Formation potential of tropospheric ozone photochemical oxidants; ADPE = Abiotic depletion potential for non-fossil
resources; ADPF = Abiotic depletion potential for fossil resources; WDP = Water (user) deprivation potential)
RESULTS OF THE LCA - INDICATORS TO DESCRIBE RESOURCE USE according to EN 15804+A2: 1 piece VELUX sun tunnel
TLF 0K14 2010 for pitched roof, flexible
Parameter Unit A1-A3 A5 C1 C2 C3 C4 D
PERE MJ 3.01E+01 4.48E+01 0 1.39E-02 2.43E-01 9.37E-02 -3.72E+01
PERM MJ 4.55E+01 -4.47E+01 0 0 -7.61E-01 0 0
PERT MJ 7.3E+01 2.34E-02 0 1.39E-02 -5.18E-01 9.37E-02 -3.72E+01
PENRE MJ 5.98E+02 3.75E+00 0 9.84E-01 1.54E-06 8.39E+01 -2.86E+02
PENRM MJ 8.48E+01 -2.12E+00 0 0 0 -8.26E+01 0
PENRT MJ 6.36E+02 1.63E+00 0 9.84E-01 1.54E-06 1.25E+00 -2.86E+02
SM kg 1.11E+00 0 0 0 0 0 1.2E+00
RSF MJ 0 0 0 0 0 0 0
NRSF MJ 0 0 0 0 0 0 0
FW m3 4.18E-01 2.02E-04 0 1.07E-04 4.59E-04 2.6E-03 -1.8E-01
PERE = Use of renewable primary energy excluding renewable primary energy resources used as raw materials; PERM = Use of renewable primary
energy resources used as raw materials; PERT = Total use of renewable primary energy resources; PENRE = Use of non-renewable primary energy
excluding non-renewable primary energy resources used as raw materials; PENRM = Use of non-renewable primary energy resources used as raw
materials; PENRT = Total use of non-renewable primary energy resources; SM = Use of secondary material; RSF = Use of renewable secondary fuels;
NRSF = Use of non-renewable secondary fuels; FW = Use of net fresh water
RESULTS OF THE LCA – WASTE CATEGORIES AND OUTPUT FLOWS according to EN 15804+A2:
1 piece VELUX sun tunnel TLF 0K14 2010 for pitched roof, flexible
Parameter Unit A1-A3 A5 C1 C2 C3 C4 D
HWD kg 4.86E-03 4.19E-06 0 2.51E-06 1.54E-06 4.2E-06 3.22E-03
NHWD kg 1.52E+01 1.11E-01 0 6.59E-02 7.83E-03 1.83E+00 -8.13E+00
RWD kg 3.53E-03 2.35E-05 0 1.42E-05 1.74E-05 9.91E-06 -9.3E-04
CRU kg 0 0 0 0 0 0 0
MFR kg 1.17E+00 2.67E+00 0 0 2.12E+00 0 0
MER kg 0 0 0 0 0 0 0
EEE MJ 2.81E-01 2.75E-01 0 0 0 1.07E+01 0
6 Environmental Product Declaration - VELUX A/S - VELUX sun tunnel TLF for pitched roof, flexible
EET MJ 5.41E-01 5.41E-01 0 0 0 2.11E+01 0
HWD = Hazardous waste disposed; NHWD = Non-hazardous waste disposed; RWD = Radioactive waste disposed; CRU = Components for re-use;
MFR = Materials for recycling; MER = Materials for energy recovery; EEE = Exported electrical energy; EET = Exported thermal energy
RESULTS OF THE LCA – additional impact categories according to EN 15804+A2-optional:
1 piece VELUX sun tunnel TLF 0K14 2010 for pitched roof, flexible
Parameter Unit A1-A3 A5 C1 C2 C3 C4 D
Disease
PM 3.74E-06 1.18E-08 0 7.06E-09 8.39E-09 1.08E-08 -2.26E-06
incidence
IR kBq U235 eq 1.37E+00 7.08E-03 0 4.27E-03 6.68E-03 4.56E-03 -3.63E-01
ETP-fw CTUe 1.1E+03 1.55E+00 0 7.79E-01 1.13E+00 1.39E+01 -5.81E+02
HTP-c CTUh 1.35E-07 7.04E-11 0 3.11E-11 3.06E-11 1.04E-09 -5.11E-08
HTP-nc CTUh 9.61E-07 1.63E-09 0 8.97E-10 9.95E-10 9.8E-09 -4.9E-07
SQP SQP 2.51E+02 1.39E+00 0 8.39E-01 2.6E-01 8.34E-01 -4.56E+01
PM = Potential incidence of disease due to PM emissions; IR = Potential Human exposure efficiency relative to U235; ETP-fw = Potential comparative
Toxic Unit for ecosystems; HTP-c = Potential comparative Toxic Unit for humans (cancerogenic); HTP-nc = Potential comparative Toxic Unit for humans
(not cancerogenic); SQP = Potential soil quality index
Disclaimer 1 – for the indicator “Potential Human exposure efficiency relative to U235”.This impact category deals mainly with the
eventual impact of low dose ionizing radiation on human health of the nuclear fuel cycle. It does not consider effects due to possible
nuclear accidents, occupational exposure or radioactive waste disposal in underground facilities. Potential ionizing radiation from the
soil, radon and from some construction materials is also not measured by this indicator.
Disclaimer 2 – for the indicators “abiotic depletion potential for non-fossil resources”, “abiotic depletion potential for fossil resources”,
“water (user) deprivation potential, deprivation-weighted water consumption”, “potential comparative toxic unit for ecosystems”,
“potential comparative toxic unit for humans – cancerogenic”, “Potential comparative toxic unit for humans - not cancerogenic”,
“potential soil quality index”. The results of this environmental impact indicator shall be used with care as the uncertainties on these
results are high as there is limited experience with the indicator.
6. LCA: Interpretation
Figure 1 illustrates the relative contributions of the different A1-A3 = 100%).
modules along the life cycle of the declared products (Modules
5% and -60%.
Figure 1: Relative environmental impacts of the different The net positive impact ('load') of the ADPelements is related to
life cycle stages for the VELUX sun tunnel TLF 0K14 2010 copper input as the copper cathode for the remelting of
(Modules A1-A3 = 100%) recycled aluminium.
The use of renewable primary energy is mainly caused by the
The LCA is dominated by the manufacture of the product share of renewable energy in the electricity mix, thus the
(modules A1-A3); further relevant contributions come only from production stage is the main driver of this impact category; the
the incineration of the plastic waste in module C4. same holds also for the use of non-renewable primary energy.
The benefits and burdens outside the product system vary in Material use of primary energy is negligible and related to
significance depending on the indicator and fluctuate between - plastic parts of the product and packaging material. The
7 Environmental Product Declaration - VELUX A/S - VELUX sun tunnel TLF for pitched roof, flexible
material use of primary energy is transferred to its energy use flows is mainly caused during mining andprocessing of metal
when the materials containing primary energy are incinerated ores and related to the disposal of road infrastructure;
with energy recovery. hazardous and radioactive waste are mainly caused by the
Non-hazardous waste as the quantitatively most relevant waste nuclear power in the electricity mix.
7. Requisite evidence
8.1 Formaldehyde standard.
Not tested based on applicable product standard.
7.2 MDI 7.4. Fire gas toxicity
Not tested based on applicable product standard. Not tested based on applicable product standard.
7.3 Checking of pre-treatment of substances used 7.5 VOC emissions
according to AltholzVO Not tested based on applicable product standard.
Not applicable; not tested based on applicable product
8. References
Product category rules of IBU ISO 14001
DIN EN ISO 14001:2015: Environmental management
IBU (2021) systems - Requirements with guidance for use.
IBU (2021): General Instructions for the EPD Programme of the
Institut Bauen und Umwelt e.V.. Version 2.0, Institut Bauen und ISO 45001
Umwelt e.V., Berlin ISO 45001:2018-03, Occupational health and safety
management systems - Requirements with guidance for use.
IBU (2022)
IBU (2022): Product category rules for building-related products EN 1873
and service, PCR Part A: Calculation rules for the life cycle DIN EN 1873:2005, Prefabricated accessories for roofing -
assessment and requirements for the project report. Version Individual rooflights of plastics - product specification and test
2.2., Institut Bauen und Umwelt e.V., Berlin. methods.
IBU (2023) ECHA candidate list
IBU (2023): PCR Guidance-Texts for Building-Related Products The Candidate List of Substances of Very High Concern for
and Services, PCR Part B: Requirements on the EPD for Authorisation, European Chemicals Agency, Helsinki.
windows and doors. Version 2023/04, Institut Bauen und
Umwelt e.V., Berlin. Regulation on biocidal products
REGULATION (EU) No 528/2012 OF THE EUROPEAN
Standards and legal documents PARLIAMENT AND OF THE COUNCIL of 22 May 2012
concerning the making available on the market and use of
EN 15804 biocidal products.
DIN EN 15804+A2:2022-3, Sustainability of construction
works - Environmental product declarations - Core rules for the Regulation (EU) Nr. 305/2011(CPR)
product category construction products. German version EN REGULATION (EU) No 305/2011 OF THE EUROPEAN
15804:2012+A2:2019 + AC:2021 PARLIAMENT AND OF THE COUNCIL of 9 March 2011 laying
down harmonised conditions for the marketing of construction
ISO 14025 products and repealing Council Directive 89/106/EEC.
DIN EN ISO 14025:2006-07, Environmental labels and
declarations - Type III Environmental declarations - Principles COUNCIL REGULATION (EU) No 333/2011
and procedures. COUNCIL REGULATION (EU) No 333/2011 of 31 March 2011
establishing criteria determining when certain types of scrap
ISO 14044 metal cease to be waste under Directive 2008/98/EC of the
DIN EN ISO 14044:2006-07, Environmental management - Life European Parliament and of the Council.
cycle assessment - Requirements and guidance (ISO
14044:2006); German and English versions EN ISO European Waste List (Waste index)
14044:2006. http://www.gesetze-im-internet.de/avv/anlage.htm
ISO 9001 Additional references
DIN EN ISO 9001:2015, Quality management systems -
Requirements. ecoinvent 3.8
ecoinvent 3.8, LCA database, 12/2021. Ecoinvent centre,
Zürich.
8 Environmental Product Declaration - VELUX A/S - VELUX sun tunnel TLF for pitched roof, flexible
Publisher
Institut Bauen und Umwelt e.V. +49 (0)30 3087748- 0
Hegelplatz 1 info@ibu-epd.com
10117 Berlin www.ibu-epd.com
Germany
Programme holder
Institut Bauen und Umwelt e.V. +49 (0)30 3087748- 0
Hegelplatz 1 info@ibu-epd.com
10117 Berlin www.ibu-epd.com
Germany
Author of the Life Cycle Assessment
Dr. Frank Werner - Umwelt & Entwicklung + 41 (0)44 241 39 06
Kammelenbergstrasse 30 frank@frankwerner.ch
9011 St. Gallen http://www.frankwerner.ch/
Switzerland
Owner of the Declaration
VELUX Group +4545164726
Ådalsvej 99 jakob.roerbech@velux.com
2970 Hørsholm www.velux.com
Denmark
9 Environmental Product Declaration - VELUX A/S - VELUX sun tunnel TLF for pitched roof, flexible
