ENVIRONMENTAL PRODUCT DECLARATION
as per ISO 14025 and EN 15804+A2
Owner of the Declaration CELO Befestigungssysteme GmbH
Publisher Institut Bauen und Umwelt e.V. (IBU)
Programme holder Institut Bauen und Umwelt e.V. (IBU)
Declaration number EPD-CLO-20240120-CAA1-EN
Issue date 03.04.2024
Valid to 16.01.2028
ResiFIX VYSF
CELO Befestigungssysteme GmbH
www.ibu-epd.com | https://epd-online.com
General Information
CELO Befestigungssysteme GmbH ResiFIX VYSF
Programme holder Owner of the declaration
IBU – Institut Bauen und Umwelt e.V. CELO Befestigungssysteme GmbH
Hegelplatz 1 Industriestraße 6
10117 Berlin 86551 Aichach
Germany Germany
Declaration number Declared product / declared unit
EPD-CLO-20240120-CAA1-EN The declared product is the two-component reaction resin mortar "ResiFIX
VYSF", manufacturated by CELO Befestigungssysteme GmbH. The
declared unit is based on 1 kg reaction resin product in the ratio at which
the two components must be mixed before use. The packaging is also
included in the calculation, since the product is sold by CELO
Befestigungssysteme GmbH with its packaging. The declared unit is
indicated in [kg].
This declaration is based on the product category rules: Scope:
Reaction resin products, 01.08.2021 This document covers the two-component reaction resin mortar "ResiFIX
(PCR checked and approved by the SVR) VYSF". To prepare the life cycle assessment [LCA], specific data were
collected from theCELO Befestigungssysteme GmbH manufacturing
facility in CELO Befestigungssysteme GmbH, Plant2 Germany. The
Issue date assessment is based on data from 2020 which correspond to the yearly
average. The procedure by which the data are allocated to the declared
03.04.2024
unit is described in the "Allocation" section.
Valid to
16.01.2028
The owner of the declaration shall be liable for the underlying information
and evidence; the IBU shall not be liable with respect to manufacturer
information, life cycle assessment data and evidences.
The EPD was created according to the specifications of EN 15804+A2. In
the following, the standard will be simplified as EN 15804.
Verification
The standard EN 15804 serves as the core PCR
Independent verification of the declaration and data according to ISO
14025:2011
Dipl.-Ing. Hans Peters
(Chairman of Institut Bauen und Umwelt e.V.) internally X externally
Florian Pronold Angela Schindler,
(Managing Director Institut Bauen und Umwelt e.V.) (Independent verifier)
1 Environmental Product Declaration - CELO Befestigungssysteme GmbH - ResiFIX VYSF
Product
-10°C 90 min.
Product description/Product definition -5°C 90 min.
The declared product ResiFIX VYSF is a two-component 0°C 45 min.
reaction resin mortar based on vinyl ester resin that is delivered +5°C 25 min.
in a two-component plastic cartridge. The high-performance +10°C 15 min.
product is applied through a static mixer using a manual, +20°C 6 min.
battery-operated or pneumatic gun. It was specially developed +30°C 4 min.
for use in securing threaded rods, rebar or internally threaded +35°C 2 min.
sleeves in solid brick, concrete, autoclaved aerated concrete +40°C 1.5 min.
and lightweight concrete. Due to its excellent mechanical
strength, it can also be used in perforated brick by using a Curing time in dry substrate:
special perforated sleeve. ResiFIX VYSF mortar has a wide -10°C 1440 min.
range of possible applications at installation tempeartures as -5°C 840 min.
low as -10 °C and operating temperatures of up to 120 °C, and 0°C 420 min.
offers high chemical resistance in extreme environments like +5°C 120 min.
swimming pools (chlorine) or near the sea (salt). With its broad +10°C 80 min.
range of national and international approvals and certifications, +20°C 45 min.
it can be used in almost any application. +30°C 25 min.
+35°C 20 min.
Marketing of the product in the EU/EFTA (except for +40°C 15 min.
Switzerland) is governed by Regulation (EU) No. 305/2011
(CPR). The product requires a Declaration of Performance
subject to ETA-10/0134, ETA-15/0320, ETA-13/0315 and CE
marking. For more information, please refer to the relevant technical data
sheet.
Product performance values in accordance with the Declaration
Application
of Performance with regard to its principal charateristics
The declared product ResiFIX VYSF is used to reliably secure according to ETA-10/0134, ETA-15/0320 and ETA-13/0315.
threaded rods, internally threaded sleeves and post-installed
rebar connections in dry and moist concrete or masonry. The Base materials/Ancillary materials
ResiFIX VYSF product can also be used for water-filled The declared product ResiFIX VYSF is delivered as a two-
boreholes. The declared product ResiFIX VYSF has very good component plastic cartridge and consists of a resin component
mechanical and thermal properties as well as very high and a curing agent component in a 10:1 volume ratio. The
chemical resistance. It can be used in aggressive mixing ratio between the resin component and the curing agent
environments. The declared product ResiFIX VYSF emits only component is set automatically as the product is pushed out of
a slight odour. the cartridge. Curing begins immediately after the components
are mixed.
Sample applications
Suitable for securing façades, canopies, wooden structures,
metal structures, metal profiles, supports, beams, panels, 1) "This product/article/at least one partial article contains
railings, gratings, plumbing fixtures, pipes, cable trays, post- substances in the ECHA candidate list of substances of very
installed rebar connections (for renovations or reinforcement), high concern (SVHC) (10 June 2022) above a concentration of
etc. 0.1% by mass: no."
Technical Data
The following construction data are relevant for the declared
product ResiFIX VYSF as delivered: 2) "This product/article/at least one partial article contains other
Construction data CMR substances in categories 1A or 1B which are not on the
candidate list, exceeding 0.1 percentage by mass: no"
Name Value Unit
Density acc. to DIN 51757 for mixing the two
1.6 g/ml
components
Compressive strength acc. to DIN EN 196 Part 1 100.6N/mm² 3)"Biocide products were added to this construction product or
Flexural strength acc. to DIN EN 196 Part 1 14.7 N/mm² it has been treated with biocide products (this then concerns a
treated product as defined by the (EU) Regulation on Biocidal
Products No. 528/2012): no"
Storage:
Store in a cool, dry and dark place; storage temperature: +5°C
to +25°C
The product considered in this EPD contains individual
components in the following ranges:
Shelf life:
18 months in standard cartridge systems
18 months in foil tube cartridge systems
Resin component:
Gel and working time:
Vinyl ester resin: 30 to 40% by weight
2 Environmental Product Declaration - CELO Befestigungssysteme GmbH - ResiFIX VYSF
Other components: 10 to 35% by weight
Mineral fillers: 50 to 70% by weight
Reference service life
Other components: < 5% by weight The declared product ResiFIX VYSF may be exposed to a wide
range of environmental conditions during the use phase. Its
expected reference service life depends on the specific
installation situation and on the product's resulting exposure.
Curing agent component: The main factors influencing service life are weather conditions
Dibenzoyl peroxide: 10 to 15% by weight and mechanical and chemical stresses.
Mineral fillers: 40 to 60% by weight
LCA: Calculation rules
The precursor products are sourced from Germany, England
Declared Unit and France, Transport is mainly done by truck. Only the
The product declared is a two-component reaction resin mortar transport from England is done by rail. The following process
manufactured by CELO Befestigungssysteme GmbH with the diagrams illustrate the underlying production process.
product name ResiFIX VYSF. The declared unit is based on 1
kg reaction resin product in the ratio at which the two
components must be mixed before use.
The mixing ratio between the resin component and the curing
agent component is 9:1 [m/m] (volume ratio 10:1). The
packaging is also included in the calculation at 0.3013 kg per 1
kg of reaction resin product. The declared unit data are
presented in the table below.
Declared unit data
Name Value Unit
Declared unit 1 kg
System boundary
Type of EPD: Cradle to factory gate with options. The following
information modules are defined as system boundaries in this
study:
Figure 1 Information modules A 1 to A3 of the product
Production stage (A1- A3):
• A1, Raw material extraction,
• A2, Transport to the manufacturer,
• A3, Manufacturing.
End of life (C1- C4):
C1, Deconstruction/demolition, Figure 2 Information modules A 1 to A3 of the packaging
C2, Transport,
Geographic Representativeness
C3, Waste processing,
Land or region, in which the declared product system is
C4, Disposal.
manufactured, used or handled at the end of the product´s
lifespan: Germany
Reuse, recovery and recycling potential (D)
To precisely determine the indicators and environmental
Comparability
impacts of the declared unit, a total of 8 information modules
Basically, a comparison or an evaluation of EPD data is only
are considered. The information modules A1 to A3 describe the
possible if all the data sets to be compared were created
material provision, the transport to the production site, as well
according to EN 15804 and the building context, respectively
as the production processes of the product itself.
the product-specific characteristics of performance, are taken
into account.
LCA: Scenarios and additional technical information
Packaging per declared unit
Characteristic product properties of biogenic carbon
No renewable raw materials are used in the product or the Name Value Unit
packaging. The biogenic carbon value is therefore reported as Packaging PP 0.0318 kg
zero. Packaging PA6 0.2696 kg
3 Environmental Product Declaration - CELO Befestigungssysteme GmbH - ResiFIX VYSF
End of Life (C1-C4) Reuse, recovery and recycling potential (D), relevant
The product is demolished by using an electric chisel. The scenario specifications
electrical energy consumption for this tool is estimated at 0.05 The product has no reuse, recovery or recycling potential.
MJ for the declared unit. The power consumption is calculated Information module D is therefore declared and reported as
using a European energy mix. Construcion waste is transported zero.
200 km by truck to a waste treatment facility. At the waste Name Value Unit
treatment facility, the construction waste is shredded and the
Reuse, recovery and recycling potential 0 kg
disposed of in a landfill.
Name Value Unit
Collected as mixed construction waste 1 kg
Shredding 1 kg
Disposal in landfill 1 kg
4 Environmental Product Declaration - CELO Befestigungssysteme GmbH - ResiFIX VYSF
LCA: Results
DESCRIPTION OF THE SYSTEM BOUNDARY (X = INCLUDED IN LCA; MND = MODULE OR INDICATOR NOT DECLARED; MNR
= MODULE NOT RELEVANT)
Benefits and
Construction loads beyond
Product stage Use stage End of life stage
process stage the system
boundaries
la ire ta m w a Ry lp p u s tro p s n a rT g n iru tc a fu n a M e h t m o rf tro p s n a rTe tis e h t o t e ta g y lb m e s s A e s U e c n a n e tn ia M ria p e R tn e m e c a lp e R tn e m h s ib ru fe R y g re n e la n o ita re p Oe s u re ta w la n o ita re p Oe s u n o itc u rts n o c -e Dn o itilo m e d tro p s n a rT g n is s e c o rp e ts a W la s o p s iD -e s u e R-y re v o c e R-g n ilc y c e Rla itn e to p
A1 A2 A3 A4 A5 B1 B2 B3 B4 B5 B6 B7 C1 C2 C3 C4 D
X X X MND MND MND MND MNR MNR MNR MND MND X X X X X
RESULTS OF THE LCA - ENVIRONMENTAL IMPACT according to EN 15804+A2: 1 kg ResiFIX VYSF
Parameter Unit A1-A3 C1 C2 C3 C4 D
Global Warming Potential total (GWP-total) kg CO 2 eq 4.68E+00 5.12E-03 1.51E-02 2.6E-03 1.45E-02 0
Global Warming Potential fossil fuels (GWP-fossil) kg CO 2 eq 4.68E+00 5.12E-03 1.5E-02 2.59E-03 1.45E-02 0
Global Warming Potential biogenic (GWP-biogenic) kg CO 2 eq 0 0 0 0 0 0
Global Warming Potential luluc (GWP-luluc) kg CO 2 eq 8E-04 1.08E-06 8.28E-05 1.2E-05 2.67E-05 0
Depletion potential of the stratospheric ozone layer (ODP) kg CFC11 eq 6.24E-09 7.5E-14 8.9E-16 3.85E-15 3.4E-14 0
Acidification potential of land and water (AP) mol H+ eq 7.09E-03 1.12E-05 4.67E-05 1.34E-05 1.03E-04 0
Eutrophication potential aquatic freshwater (EP-freshwater) kg P eq 2.57E-05 1.49E-08 4.43E-08 7.43E-09 2.45E-08 0
Eutrophication potential aquatic marine (EP-marine) kg N eq 2.29E-03 2.52E-06 2.15E-05 6.11E-06 2.62E-05 0
Eutrophication potential terrestrial (EP-terrestrial) mol N eq 2.1E-02 2.65E-05 2.4E-04 6.74E-05 2.88E-04 0
Formation potential of tropospheric ozone photochemical oxidants kg NMVOC
6.57E-03 6.82E-06 4.22E-05 1.66E-05 7.97E-05 0
(POCP) eq
Abiotic depletion potential for non fossil resources (ADPE) kg Sb eq 1.14E-06 1.4E-09 1.24E-09 2.87E-09 1.48E-09 0
Abiotic depletion potential for fossil resources (ADPF) MJ 9.01E+01 9.29E-02 1.98E-01 5.06E-02 1.9E-01 0
m3 world eq
Water use (WDP) 1.49E-01 1.17E-03 1.33E-04 4.99E-04 1.59E-03 0
deprived
RESULTS OF THE LCA - INDICATORS TO DESCRIBE RESOURCE USE according to EN 15804+A2: 1 kg ResiFIX VYSF
Parameter Unit A1-A3 C1 C2 C3 C4 D
Renewable primary energy as energy carrier (PERE) MJ 1.17E+01 5.16E-02 1.13E-02 4.06E-03 2.85E-02 0
Renewable primary energy resources as material utilization
MJ 0 0 0 0 0 0
(PERM)
Total use of renewable primary energy resources (PERT) MJ 1.17E+01 5.16E-02 1.13E-02 4.06E-03 2.85E-02 0
Non renewable primary energy as energy carrier (PENRE) MJ 6.07E+01 9.3E-02 1.99E-01 5.07E-02 1.9E-01 0
Non renewable primary energy as material utilization (PENRM) MJ 2.95E+01 0 0 0 0 0
Total use of non renewable primary energy resources (PENRT) MJ 9.02E+01 9.3E-02 1.99E-01 5.07E-02 1.9E-01 0
Use of secondary material (SM) kg 0 0 0 0 0 0
Use of renewable secondary fuels (RSF) MJ 0 0 0 0 0 0
Use of non renewable secondary fuels (NRSF) MJ 0 0 0 0 0 0
Use of net fresh water (FW) m3 1.33E-02 4.92E-05 1.28E-05 1.42E-05 4.82E-05 0
RESULTS OF THE LCA – WASTE CATEGORIES AND OUTPUT FLOWS according to EN 15804+A2:
1 kg ResiFIX VYSF
Parameter Unit A1-A3 C1 C2 C3 C4 D
Hazardous waste disposed (HWD) kg 9.76E-09 8.04E-12 9.53E-13 6.34E-13 9.75E-12 0
Non hazardous waste disposed (NHWD) kg 8.53E-02 7E-05 2.85E-05 1.34E-05 9.71E-01 0
Radioactive waste disposed (RWD) kg 1.33E-03 1.49E-05 2.45E-07 6.68E-07 2.11E-06 0
Components for re-use (CRU) kg 0 0 0 0 0 0
Materials for recycling (MFR) kg 0 0 0 0 0 0
Materials for energy recovery (MER) kg 0 0 0 0 0 0
Exported electrical energy (EEE) MJ 0 0 0 0 0 0
Exported thermal energy (EET) MJ 0 0 0 0 0 0
RESULTS OF THE LCA – additional impact categories according to EN 15804+A2-optional:
1 kg ResiFIX VYSF
Parameter Unit A1-A3 C1 C2 C3 C4 D
Disease
Incidence of disease due to PM emissions (PM) ND ND ND ND ND ND
incidence
Human exposure efficiency relative to U235 (IR) kBq U235 eq ND ND ND ND ND ND
Comparative toxic unit for ecosystems (ETP-fw) CTUe ND ND ND ND ND ND
Comparative toxic unit for humans (carcinogenic) (HTP-c) CTUh ND ND ND ND ND ND
Comparative toxic unit for humans (noncarcinogenic) (HTP-nc) CTUh ND ND ND ND ND ND
5 Environmental Product Declaration - CELO Befestigungssysteme GmbH - ResiFIX VYSF
Soil quality index (SQP) SQP ND ND ND ND ND ND
The dataset "DE: Epoxy Resin, Source: Sphera, Reference year: 2021" was updated with reference to the previous EPD. As this
dataset has a strong influence on the overall calculation, the results are higher in comparison to the previous EPD from 2015.
References
Standards ETA-10/0134
European Technical Assessment CELO ResiFIX VYSF.
DIN 51757
DIN 51757:2011-01 ETA-15/0320
Testing of mineral oils and related materials - Determination of European Technical Assessment CELO ResiFIX VYSF.
density
ETA-13/0315
EN 196 European Technical Assessment CELO ResiFIX VYSF.
DIN EN 196-1:2016-11
Test methods for cement - Part 1: Determination of strength IBU 2021
German version EN 196-1:2016 Institut Bauen und Umwelt e.V.: General guidance for the EPD
programme of the Institut Bauen und Umwelt e.V., Version 2.0,
EN 15804 Berlin: Institut Bauen und Umwelt e.V., 2021.
EN 15804:2019-04+A2, Sustainability of construction works - www.ibu-epd.com
Environmental Product Declarations - Core rules for the product
category of construction products. PCR PART A
Product Category Rules for Building-Related Products and
ISO 14025 Services - Calculation Rules for the Life Cycle Assessment and
DIN EN ISO 14025:2011-10, Environmental labels and requirements on the Project Report V2.1, Institut Bauen und
declarations - Type III environmental declarations - Principles Umwelt e.V., 11.2021.
and procedures.
PCR: Reaction resin products
ISO 14044 Guidance-Texts for Building-Related Products and Services.
DIN EN ISO 14044:2006-10, Environmental management - Life Part B: Requirements on the EPD for Reaction resin products,
cycle assessment - Requirements and guidelines. Version 1.3. Berlin: Institut Bauen und Umwelt e.V.
(Hrsg.),07.2014.
Further references Sphera
GaBi 10 Software: Life Cycle Assessment
Leinfelden-Echterdingen; Sphera Solution GmbH (Hrsg.).
ecoinvent 3.7.1 http://www.gabi-software.com/deutsch/index/
Background database: ecoinvent 3.7.1 (25/03/2022)
Zürich: ecoinvent (Ed.) .
http://www.ecoinvent.org
(25/03/2022) Regulation (EU) No. 305/2011 (CPR)
Regulation (EU) No. 528/2012 (Biocidal Product Regulation)
6 Environmental Product Declaration - CELO Befestigungssysteme GmbH - ResiFIX VYSF
Publisher
Institut Bauen und Umwelt e.V. +49 (0)30 3087748- 0
Hegelplatz 1 info@ibu-epd.com
10117 Berlin www.ibu-epd.com
Germany
Programme holder
Institut Bauen und Umwelt e.V. +49 (0)30 3087748- 0
Hegelplatz 1 info@ibu-epd.com
10117 Berlin www.ibu-epd.com
Germany
Author of the Life Cycle Assessment
FIT-Umwelttechnik GmbH 05362 72 69 474
Westerstr. 13 bertram@fit-umwelttechnik.de
38442 Wolfsburg www.fit-umwelttechnik.com
Germany
Owner of the Declaration
CELO Befestigungssysteme GmbH +49 08251 904850
Industriestraße 6 info@celofixings.de
86551 Aichach www.celofixings.de
Germany
7 Environmental Product Declaration - CELO Befestigungssysteme GmbH - ResiFIX VYSF
