ENVIRONMENTAL PRODUCT DECLARATION
as per ISO 14025 and EN 15804+A2
Owner of the Declaration DuPont de Nemours (Luxembourg) s.à r.l.
Programme holder Institut Bauen und Umwelt e.V. (IBU)
Publisher Institut Bauen und Umwelt e.V. (IBU)
Declaration number EPD-DUP-20210189-IBC1-EN
Issue date 30.11.2021
Valid to 29.11.2026
DuPont™ Tyvek® Monolayer 70 (1570B)
DuPont de Nemours (Luxembourg) s.à r.l.
www.ibu-epd.com | https://epd-online.com
Umwelt Produktdeklaration Name des Herstellers – Name des Produkts
1. General Information
DuPont de Nemours (Luxembourg) s.à r.l. DuPontTM Tyvek® Monolayer 70
(1570B)
Programme holder Owner of the declaration
IBU – Institut Bauen und Umwelt e.V. DuPont de Nemours (Luxembourg) s.à r.l.
Panoramastr. 1 Rue Général Patton
10178 Berlin L-2984 Contern
Germany Luxembourg
Declaration number Declared product / declared unit
EPD-DUP-20210189-IBC1-EN 1 m² DuPont™ Tyvek® Monolayer (1570B)
This declaration is based on the product Scope:
category rules: This document applies to DuPont™ Tyvek® 1570B
False ceiling and underlay sheeting, 11.2017 monolayer high density polyethylene (HDPE)
(PCR checked and approved by the SVR) membranes manufactured by DuPont in L-2984
Contern, with a declared unit weight of 69 g/m2. The
LCA data were compiled using production data from
Issue date
the year 2019 by DuPont Luxembourg s.à r.l. The
30.11.2021
declaration holder is responsible for the underlying
data and its verification.
Valid to
29.11.2026
The owner of the declaration shall be liable for the
underlying information and evidence; the IBU shall not
be liable with respect to manufacturer information, life
cycle assessment data and evidences.
The EPD was created according to the specifications
of EN 15804+A2. In the following, the standard will be
simplified as EN 15804.
Verification
The standard EN 15804 serves as the core PCR
Independent verification of the declaration and data
according to ISO 14025:2010
Dipl. Ing. Hans Peters internally x externally
(chairman of Institut Bauen und Umwelt e.V.)
Dr. Alexander Röder Vito D'Incognito
(Managing Director Institut Bauen und Umwelt e.V.)) (Independent verifier)
2. Product
2.1 Product description/Product definition installed below Tyvek® is kept dry and performs as
DuPont™ Tyvek® is a nonwoven material made of designed.
HDPE, which is diffusion open but watertight. It is used
as a roof and wall underlay. 2.3 Technical Data
For the placing on the market of the product in the The following chapter comprises technical data for the
European Union/European Free Trade Association characteristics listed in the Declaration of Performance
(EU/EFTA) (with the exception of Switzerland) according to the harmonized technical specifications
Regulation (EU) No. 305/2011 (CPR) applies. The EN 13859-1 and EN 13859-2.
product needs a declaration of performance taking into
consideration EN 13859-1:2010 Flexible sheets for Constructional data
waterproofing - Definitions and characteristics of Name Value Unit
underlays - Part 1: Underlays for discontinuous roofing 50m
Length * acc. to EN 1848-2 m
and EN 13859-2:2010 Flexible sheets for standard
waterproofing - Definitions and characteristics of 1.3m
underlays - Part 2 Underlays for walls and the CE- standard
marking. For the application and use the respective 2.8m
Width * acc. to EN 1848-2 m
national provisions apply. standard
2.2 Application 3.0m
Tyvek® underlays are used in roofs and walls. They standard
constitute the second water shedding layer and at the Grammage * acc. to EN 1849-2 0.069 kg/m2
same time protect the insulation from trapped Resistance to water penetration
W1 -
moisture, wind penetration, dust and insects. Insulation acc. to EN 1928 (class)
2 Environmental Product Declaration DuPont de Nemours (Luxembourg) s.à.r.l – Tyvek® Monolayer 70 (1570B)
Water vapor diffusion equivalent wrapped in foil (LDPE: low density PE) and stacked on
air layer thickness acc. to EN ISO 0.021 m wooden pallets which are also wrapped in LDPE
12572 stretch film. Vertical sides of the pallets are protected
Maximum tensile force acc. to EN with a carton profile.
205 - 170 N/50mm
12311-1 All packaging materials can be reused (e.g. pallets),
Elongation acc. to EN 12311-1 9 - 13 % recycled or valorised through energy recovery.
Tear Resistance (nail) acc. to EN
80 - 80 N/mm
12310-1
Resistance to water penetration 2.10 Condition of use
after ageing acc. to EN 1297, EN W1 - Materials are not expected to change or react during
1928 (class) the period of use. Tyvek® is intended to be installed on
* Not listed in the declaration of performance the cold side of the insulation and is designed to
withstand substantial temperature changes during
service life.
Performance data of the product in accordance with
the declaration of performance with respect to its
2.11 Environment and health during use
essential characteristics according to EN 13859-
Tyvek® membranes are usually concealed below roof
1:2010 Flexible sheets for waterproofing - Definitions
decking or facade cladding. They do not require
and characteristics of underlays - Part 1: Underlays for
maintenance and will not produce emissions. There
discontinuous roofing and EN 13859-2:2010 Flexible
are no environmental or health concerns to be
sheets for waterproofing - Definitions and
expected from the use of the material.
characteristics of underlays - Part 2 Underlays for
walls.
2.12 Reference service life
2.4 Delivery status The documentation of the RSL is not required for this
EPD since not the entire life cycle is declared (without
The single selling unit is a roll of up to 3 m width and a
modules B1-B7). Nevertheless, the product is
length of up to 100 m. Usually several rolls are
assumed to have a reference service life of 30 years,
strapped and piled on a wooden pallet.
corresponding to the average roof lifetime (BNB
The order unit is square meter [m²].
Nutzungsdauerliste). But this assumption could not be
verified because the Tyvek® envelopes have only
2.5 Base materials/Ancillary materials
been sold for 25 years.
Tyvek® single layer membranes are made of
Influences on ageing when applied in accordance with
- high density polyethylene (HDPE) >99 %
the rules of technology
- hindered amine light stabilizers (HALS, added for UV
stabilization) <1 %.
2.6 Manufacture 2.13 Extraordinary effects
Tyvek® underlays are produced on semi-continuously
Fire
operating production facilities in different countries.
Process steps include:
1. Spinning of thin HDPE filaments. Fire protection
2. Bonding of filament sheet. Name Value
Building material class acc. to E on mineral wool and
3. Printing, slitting and packaging of the finished roll
EN13501-1 wood
goods.
2.7 Environment and health during Water
manufacturing Tyvek® membranes are inherently waterproof. No part
Some of the manufacturing facilities employed in the of the product will dissolve in water nor will the product
production of Tyvek® are ISO 14001 certified. All release any toxic substances to water.
facilities comply with local regulations and DuPont
internal standards. Mechanical destruction
Particular care is taken to ensure the safety of anyone No possible impacts on the environment following
involved in the Tyvek® supply chain in line with the unforeseeable mechanical destruction are known.
DuPont safety culture: all injuries can be prevented
(goal is ZERO). 2.14 Re-use phase
The material is not intended to be re-used or recycled.
2.8 Product processing/Installation Energy recovery is possible.
Tyvek® membranes for walls and roofs can be either
installed on the construction site or in manufacturing 2.15 Disposal
facilities in case of pre-fabricated buildings. In both Disposal of the material should be made according to
instances the material is usually installed by manually national legislation. Incineration is the preferred way of
unwinding the sheet from the roll and placing it onto disposal. European Waste Codes (Commission
the designated surface. Tools required are usually a decision 2014/955/EU) for mixed construction and
knife or scissors to cut the sheet as well as a stapler to demolition waste is 17 09 04.
fix it to the construction. Refer to Tyvek® installation
guidelines for more information.
2.16 Further information
2.9 Packaging Additional information about product properties and
Tyvek® is wound onto carton cores. Each roll comes use can be found at www.building.dupont.com.Safety
with a paper insert sheet. Rolls are individually Data Sheets (SDS) or Article Information Sheets (AIS)
of the products can be found at www.dupont.com.
3 Environmental Product Declaration DuPont de Nemours (Luxembourg) s.à.r.l – Tyvek® Monolayer 70 (1570B)
3. LCA: Calculation rules
3.1 Declared Unit monolayer production), paper ink, hotmelt, paper, tape
This declaration applies to 1 m2 of DuPont™ Tyvek® and detergent for finishing process (sum < 0.2 % of
1570B membranes, with a declared unit weight of 69 total input mass for finishing process). Transports were
g/m2. considered for all inputs and outputs. Manufacturing of
the production machines and systems and associated
Declared unit infrastructure were not taken into account in the life
Name Value Unit cycle assessment (LCA). Regarding possible off-cuts
Declared unit 1 m2 during installation, the amount is lower than 5 % and
Grammage 0.069 kg/m2 therefore also neglected.
For IBU core EPDs (where clause 3.6 is part of the 3.5 Background data
EPD): for average EPDs, an estimate of the All background data for the LCA model were taken
robustness of the LCA values must be made, e.g. from the database of GaBi 10.5.0.78.
concerning variability of the production process,
geographical representativeness and the influence of 3.6 Data quality
background data and preliminary products compared To simulate the product stage, data recorded by
to the environmental impacts caused by actual DuPont Luxembourg s.à r.l. and the converting plant in
production. Germany from the production year 2019 were used.
Eurostat data for the years 2018-2019 were used to
3.2 System boundary model the modules A4 (freight transport modal split)
Type of EPD: Cradle-to-gate (with options) and A5 (packaging disposal routes).
The system boundaries of the EPD follow the modular Regarding background processes, the Luxembourg
construction system as described by EN 15804. The and German electricity grid mix were applied to the
LCA takes into account the following modules: production plants in these countries (A1-A3). Other
 A1-A3: Manufacturing of pre-products, background data were specific to Germany or the
European average, and were not older than 10 years.
packaging, ancillary materials, transport to the
The representativeness can be classified as very good
factory, production including energy supply
for all the foreground data, and most of the background
and waste handling
data.
 A4: Transport to the construction site
 A5: Installation into the building (disposal of 3.7 Period under review
packaging) The period of study encompasses the year 2019.
 C4: Waste disposal (incineration)
3.8 Allocation
 D: Potential for reuse, recovery and/or
Mass allocation was applied for production. At the
recycling (benefits for incineration and DuPont site in Luxembourg, Tyvek® waste materials
recovery of packaging materials from module are sold and transformed externally. The further use of
A5 and envelopes incineration from module the valorized HDPE granulates was cut-off from the
C3). system boundaries, as for the packaging materials
sent for recycling. The Tyvek® final waste material
sent to incineration is modelled through the
combustion process of the specific material and the
3.3 Estimates and assumptions
avoided conventional energy production is considered
The color paste used in the finishing process was
in module D. The potential benefit in module D will be
valued with a general composition of water-based color
possible only if the
paste (conservative approach).
Tyvek® will be separate and incinerated.
3.4 Cut-off criteria
3.9 Comparability
All data were taken into consideration (recipe
Basically, a comparison or an evaluation of EPD data
constituents, process water, electricity used). In case
is only possible if all the data sets to be compared
of missing data, a cut-off criteria of 1 % of the total
were created according to EN 15804 and the building
input mass was applied for unit processes and 5 % for
context, respectively the product-specific
the entire modules (as recommended by EN 15804,
characteristics of performance, are taken into account.
section 6.3.5) and therefore some inputs were
excluded: tape and spiking agent for monolayer
GaBi 10.5.0.78 was used to model background data.
production (sum < 0.04 % of total input mass for
4. LCA: Scenarios and additional technical information
Characteristic product properties product
Information on biogenic Carbon Biogenic Carbon Content in
0.0037 kg C
The product does not contain biogenic carbon. accompanying packaging
Information on describing the biogenic Carbon
Content at factury gate The following technical information serves as a basis
Name Value Unit for the declared modules or can be used for the
Biogenic Carbon Content in 0 kg C
4 Environmental Product Declaration DuPont de Nemours (Luxembourg) s.à.r.l – Tyvek® Monolayer 70 (1570B)
development of specific scenarios in the context of a
building assessment.
Transport to the building site (A4)
Name Value Unit
Transport distance 3064 km
Transport (train) 1.75E-02 tkm
Transport (road) 7.57E-02 tkm
Transport (water) 1.41E-01 tkm
Installation into the building (A5)
Name Value Unit
Wood waste to landfill 2.97E-04 kg
Wood waste to incineration 1.78E-04 kg
Cardboad waste to landfill 2.96E-04 kg
Cardboard waste to incineration 2.26E-04 kg
Plastic waste to landfill 2.66E-05 kg
Plastic waste to incineration 3.63E-05 kg
In case a reference service life according to
applicable ISO standards is declared then the
assumptions and in-use conditions underlying the
determined RSL shall be declared. In addition, it shall
be stated that the RSL applies for the reference
conditions only
The same holds for a service life declared by the
manufacturer. Corresponding information related to in-
use conditions needs not be provided if a service life
taken from the list on service life by BNB is declared.
End of life (C1-C4)
Name Value Unit
Collected separately Tyvek® waste 0.069 kg
Energy recovery 100 %
R1 value < 0.6
5 Environmental Product Declaration DuPont de Nemours (Luxembourg) s.à.r.l – Tyvek® Monolayer 70 (1570B)
5. LCA: Results
The results displayed below apply to DuPont™ Tyvek® Monolayer 70 (1570B).
Disclaimer:
EP-freshwater: This indicator has been calculated as “kg P eq” as required in the characterization model
(EUTREND model, Struijs et al., 2009b, as implemented in ReCiPe;
http://eplca.jrc.ec.europa.eu/LCDN/developerEF.xhtml).
DESCRIPTION OF THE SYSTEM BOUNDARY (X = INCLUDED IN LCA; ND = MODULE OR INDICATOR NOT
DECLARED; MNR = MODULE NOT RELEVANT)
BENEFITS AND
CONSTRUCTI LOADS
PRODUCT STAGE ON PROCESS USE STAGE END OF LIFE STAGE BEYOND THE
STAGE SYSTEM
BOUNDARIES
6 Environmental Product Declaration DuPont de Nemours (Luxembourg) s.à.r.l – Tyvek® Monolayer 70 (1570B)
lairetam
waR
ylppus tropsnarT
gnirutcafunaM
eht
morf
tropsnarT
etis
eht
ot
etag
ylbmessA esU
ecnanetniaM
riapeR
tnemecalpeR tnemhsibrufeR
ygrene
lanoitarepO esu
retaw
lanoitarepO esu
noitcurtsnoc-eD
noitilomed tropsnarT
gnissecorp
etsaW
lasopsiD -esueR -yrevoceR -gnilcyceR laitnetop
A1 A2 A3 A4 A5 B1 B2 B3 B4 B5 B6 B7 C1 C2 C3 C4 D
X X X X X ND ND MNR MNR MNR ND ND ND ND ND X X
RESULTS OF THE LCA - ENVIRONMENTAL IMPACT according to EN 15804+A2: 1 m2 m2 DuPont™
Tyvek® Monolayer 70 (1570B)
Core Indicator Unit A1-A3 A4 A5 C4 D
Global warming potential - total [kg CO2-Eq.] 3.31E-1 7.12E-3 1.85E-3 2.16E-1 -1.14E-1
Global warming potential - fossil fuels [kg CO2-Eq.] 3.31E-1 6.97E-3 1.50E-4 2.16E-1 -1.14E-1
Global warming potential - biogenic [kg CO2-Eq.] 3.60E-4 9.74E-5 1.70E-3 7.18E-6 -5.35E-4
GWP from land use and land use change [kg CO2-Eq.] 2.50E-4 4.73E-5 4.91E-8 1.16E-6 -7.18E-5
Depletion potential of the stratospheric ozone layer [kg CFC11-Eq.] 4.18E-12 5.62E-18 2.39E-19 1.62E-17 -1.18E-15
Acidification potential, accumulated exceedance [mol H+-Eq.] 1.28E-3 7.77E-5 3.89E-7 2.15E-5 -1.41E-4
Eutrophication, fraction of nutrients reaching freshwater
[kg P-Eq.] 5.12E-7 1.78E-8 3.68E-9 2.16E-9 -1.36E-7
end compartment
Eutrophication, fraction of nutrients reaching marine end
[kg N-Eq.] 2.05E-4 2.82E-5 1.70E-7 4.52E-6 -4.10E-5
compartment
Eutrophication, accumulated exceedance [mol N-Eq.] 2.21E-3 3.11E-4 1.58E-6 1.01E-4 -4.40E-4
Formation potential of tropospheric ozone photochemical
[kg NMVOC-Eq.] 7.25E-4 6.38E-5 6.85E-7 1.35E-5 -1.16E-4
oxidants
Abiotic depletion potential for non-fossil resources [kg Sb-Eq.] 5.06E-8 5.31E-10 5.04E-12 2.45E-10 -1.77E-8
Abiotic depletion potential for fossil resources [MJ] 8.28E+0 9.42E-2 8.54E-4 2.64E-2 -1.97E+0
Water (user) deprivation potential, deprivation-weighted [m³ world-Eq
3.00E-2 8.36E-5 8.61E-5 1.99E-2 -7.80E-3
water consumption (WDP) deprived]
RESULTS OF THE LCA - INDICATORS TO DESCRIBE RESOURCE USE according to EN 15804+A2: 1 m2
m2 DuPont™ Tyvek® Monolayer 70 (1570B)
Indicator Unit A1-A3 A4 A5 C4 D
Renewable primary energy as energy carrier [MJ] 7.38E-1 5.95E-3 8.75E-5 5.22E-3 -4.04E-1
Renewable primary energy resources as material utilization [MJ] 3.39E-4 -1.11E-14 -1.22E-16 2.17E-14 -8.15E-13
Total use of renewable primary energy resources [MJ] 7.38E-1 5.95E-3 8.75E-5 5.22E-3 -4.04E-1
Non-renewable primary energy as energy carrier [MJ] 8.28E+0 9.43E-2 8.54E-4 2.64E-2 -1.97E+0
Non-renewable primary energy as material utilization [MJ] 1.82E-4 3.03E-6 1.67E-8 9.33E-7 -6.38E-5
Total use of non-renewable primary energy resources [MJ] 8.28E+0 9.43E-2 8.54E-4 2.64E-2 -1.97E+0
Use of secondary material [kg] 3.62E-3 0.00E+0 0.00E+0 0.00E+0 0.00E+0
Use of renewable secondary fuels [MJ] 5.65E-8 0.00E+0 0.00E+0 0.00E+0 0.00E+0
Use of non-renewable secondary fuels [MJ] 6.23E-7 0.00E+0 0.00E+0 0.00E+0 0.00E+0
Use of net fresh water [m³] 4.16E-3 6.55E-6 2.05E-6 4.66E-4 -3.93E-4
RESULTS OF THE LCA – WASTE CATEGORIES AND OUTPUT FLOWS according to EN 15804+A2:
1 m2 m2 DuPont™ Tyvek® Monolayer 70 (1570B)
Indicator Unit A1-A3 A4 A5 C4 D
Hazardous waste disposed [kg] 1.77E-9 4.90E-12 1.54E-13 4.71E-12 -4.36E-10
Non-hazardous waste disposed [kg] 3.23E-3 1.53E-5 4.46E-4 8.57E-4 -8.63E-4
Radioactive waste disposed [kg] 1.43E-4 6.36E-7 1.79E-8 1.50E-6 -1.29E-4
Components for re-use [kg] 0.00 0.00 0.00 0.00 0.00
Materials for recycling [kg] 0.00 0.00 0.00 0.00 0.00
Materials for energy recovery [kg] 0.00 0.00 0.00 0.00 0.00
Exported electrical energy [MJ] 0.00E+0 0.00E+0 1.46E-3 4.61E-1 0.00E+0
Exported thermal energy [MJ] 0.00E+0 0.00E+0 2.08E-3 8.20E-1 0.00E+0
RESULTS OF THE LCA – additional impact categories according to EN 15804+A2-optional:
1 m2 m2 DuPont™ Tyvek® Monolayer 70 (1570B)
Indicator Unit A1-A3 A4 A5 C4 D
Potential incidence of disease due to PM emissions [Disease
ND ND ND ND ND
Incidence]
Potential Human exposure efficiency relative to U235 [kBq U235-
ND ND ND ND ND
Eq.]
Potential comparative toxic unit for ecosystems [CTUe] ND ND ND ND ND
Potential comparative toxic unit for humans - cancerogenic [CTUh] ND ND ND ND ND
Potential comparative toxic unit for humans - not cancerogenic [CTUh] ND ND ND ND ND
Potential soil quality index [-] ND ND ND ND ND
Disclaimer 1 – for the indicator “potential Human exposure efficiency relative to U235“.
This impact category deals mainly with the eventual impact of low dose ionizing
radiation on human health of the nuclear fuel cycle. It does not consider effects due to possible
nuclear accidents, occupational exposure nor radioactive waste disposal in underground
facilities. Potential ionizing radiation from the soil, radon and from some construction materials is also not
measured by this indicator.
Disclaimer 2 – for the indicators: “abiotic depletion potential for fossil resources”, “abiotic depletion potential for
non-fossil resources”, “water (user) deprivation potential”, “deprivation-weighted water consumption”, “potential
comparative toxic unit for ecosystems”, “potential comparative toxic unit for humans - cancer effects”, “potential
comparative toxic unit for humans – non-cancer effects”, “potential soil quality index”.
The results of this environmental impact indicator shall be used with care as the
uncertainties on these results are high or as there is limited experience with the indicator.
6. LCA: Interpretation
The following chart shows the relative contributions of a dominance analysis.
the different modules to the various LCA categories in
Waste incineration during the finishing step, including
For most of the impact categories, more than 70 % of Tyvek® and packaging materials, is completely
the impacts are dominated by the Tyvek® production dominating the ODP score due to halogens emissions
(A1-A3) and in particular by the supply of HDPE to air in the module „EU-28: Waste incineration of
granulates, steam and electricity. plastics (PE, PP, PS, PB)“. The transport of Tyvek®
The production phase represents 59 % of GWP, which products to the customers contributes to 12 % of MEP
is also highly influenced by the final disposal (39 % of and TEP due to the emissions of nitrogen monoxide
the generated impact). This is due to the emissions of during lorry and sea transport (module A4). As
carbon dioxide from the incineration plant. expected, the use of water, in particular cold water for
The avoided energy production thanks to waste monolayer production, dominates the WDP score.
incineration leads to significant benefits, which are
mostly around 20 % of the impact results. Glossary:
7 Environmental Product Declaration DuPont de Nemours (Luxembourg) s.à.r.l – Tyvek® Monolayer 70 (1570B)
MEP: Eutrophication, fraction of nutrients reaching
ADPE: Abiotic depletion potential for non-fossil marine end compartment
resources Mono: Monolayer production
ADPF: Abiotic depletion potential for fossil resources Nat. gas: Natural gas
AP: Acidification potential, accumulated exceedance ODP: Depletion potential of the stratospheric ozone
FEP: Eutrophication, fraction of nutrients reaching layer
freshwater end compartment POCP: Formation potential of tropospheric ozone
Fin.: Finishing process photochemical oxidants
GWP: Global Warming Potential TEP: Eutrophication, accumulated exceedance
HDPE: High-Density Polyethylene WDP: Water (user) deprivation potential, deprivation-
LCA: Life Cycle Assessment weighted water consumption
7. Requisite evidence
No requisite evidence is required for DuPont™
Tyvek® 1570B monolayer membranes.
8. References
EN 1928
EN 1928:2000, Flexible sheets for waterproofing -
EN 12310-1 Bitumen, plastic and rubber sheets for roof
EN 12310-1:1999, Flexible sheets for waterproofing - waterproofing - Determination of watertightness
Part 1: Bitumen sheets for roof waterproofing;
determination of resistance to tearing (nail shank) EN ISO 12572
EN ISO 12572:2017, Hygrothermal performance of
EN 12311-1 building materials and products -- Determination of
EN 12311-1:1999, Flexible sheets for waterproofing - water vapour transmission properties
Part 1: Bitumen sheets for roof waterproofing;
Determination of tensile properties EN ISO 14001
EN ISO 14001:2015, Environmental management
EN 1297 systems - Requirements with guidance for use (ISO
EN 1297:2004, Flexible sheets for waterproofing - 14001:2015)
Bitumen, plastic and rubber sheets for roof
waterproofing - Method of artificial ageing by long term ISO 14025
exposure to the combination of UV radiation, elevated DIN EN ISO 14025:2011-10, Environmental labels and
temperature and water declarations — Type III environmental declarations —
Principles and procedures.
EN 13501-1
EN 13501-1:2007+A1:2010, Fire classification of PCR, Part A
construction products and building elements - Part 1: PCR 2021, Part A - PCR Guidance-Calculation Rules
Classification using data from reaction to fire tests for the Life Cycle Assessment and Requirements on
the Project Report according to EN 15804+A2:2019
EN 13859-1 (version 1.1.1, 2021)
EN 13859-1:2010, Flexible sheets for waterproofing -
Definitions and characteristics of underlays - Part 1: PCR, Part B
Underlays for discontinuous roofing PCR 2017, Part B - PCR Guidance-Texts for Building-
Related Products and Services: Requirements on the
EN 13859-2 EPD for False ceiling and underlay sheeting (version
EN 13859-2:2010, Flexible sheets for waterproofing - 1.6, 2017)
Definitions and characteristics of underlays - Part 2:
Underlays for walls IBU 2016
Institut Bauen und Umwelt e.V.: General Programme
EN 15804 Instructions for the Preparation of EPDs at the Institut
EN 15804:2019+A2, Sustainability of construction Bauen und Umwelt e.V. Version 1., Berlin: Institut
works — Environmental Product Declarations — Core Bauen und Umwelt e.V., 2016. www.ibu-epd.com
rules for the product category of construction products.
BNB Nutzungsdauerliste
EN 1848-2 BNB Nutzungsdauerliste: 2017. Nutzungsdaueren von
EN 1848-2:2001, Flexible sheets for waterproofing - Bauteilen published by Informationsportal Nachhaltiges
Determination of length, width, straightness and Bauen des Bundesministeriums des Inneren für Bau
flatness - Part 2: Plastic and rubber sheets for roof und Heimat.
waterproofing
European Waste Code
EN 1849-2 European Waste Code:2000. European List of Waste
EN 1849-2:2019, Flexible sheets for waterproofing - European Waste Codes: (Commission decision
Determination of thickness and mass per unit area - 2014/955/EU)
Part 2: Plastic and rubber sheets
8 Environmental Product Declaration DuPont de Nemours (Luxembourg) s.à.r.l – Tyvek® Monolayer 70 (1570B)
Eurostat Regulation (EU) No. 305/2011 of the European
Eurostat:2021, Data browser, Packaging waste by Parliament and of the Council of 9 March 2011 laying
waste management operations; Recycling rate of down harmonised conditions for the marketing of
packaging waste by type of packaging construction products and repealing Council Directive
89/106/EEC
GaBi 10.5.0.78
GaBi 10.5.0.78:2021. Life Cycle Engineering software DuPont™, the DuPont Oval Logo, and
and database. Sphera Solutions GmbH, 2021. all trademarks and service marks denoted with ™,
SM or ® are owned by affiliates of DuPont de
Regulation (EU) No. 305/2011 Nemours, Inc. unless otherwise noted.
9 Environmental Product Declaration DuPont de Nemours (Luxembourg) s.à.r.l – Tyvek® Monolayer 70 (1570B)
Publisher
Institut Bauen und Umwelt e.V. Tel +49 (0)30 3087748- 0
Panoramastr. 1 Fax +49 (0)30 3087748- 29
10178 Berlin Mail info@ibu-epd.com
Germany Web www.ibu-epd.com
Programme holder
Institut Bauen und Umwelt e.V. Tel +49 (0)30 - 3087748- 0
Panoramastr 1 Fax +49 (0)30 – 3087748 - 29
10178 Berlin Mail info@ibu-epd.com
Germany Web www.ibu-epd.com
Author of the Life Cycle
Assessment Tel 00352-275888-1
Luxembourg Institute of Science Fax 00352-275888-555
and Technology (LIST) Mail info@list.lu
Avenue des Hauts-Fourneaux 5 Web www.list.lu
4362 Esch/Alzette
Luxembourg
Owner of the Declaration
DuPont de Nemours (Luxembourg) Tel +352 3666 5210
s.à r.l. Fax +352 3666 0000
Rue Général Patton 1 Mail tyvek.info@dupont.com
2984 Contern Web www.dupont.com
Luxembourg
