ENVIRONMENTAL PRODUCT DECLARATION
as per ISO 14025 and EN 15804+A2
Owner of the Declaration dormakaba International Holding GmbH
Publisher Institut Bauen und Umwelt e.V. (IBU)
Programme holder Institut Bauen und Umwelt e.V. (IBU)
Declaration number EPD-DOR-20220166-CBA1-EN
Issue date 17.10.2022
Valid to 16.10.2027
Kentaur
Dormakaba
www.ibu-epd.com | https://epd-online.com
General Information
Dormakaba Kentaur
Programme holder Owner of the declaration
IBU – Institut Bauen und Umwelt e.V. dormakaba International Holding GmbH
Hegelplatz 1 DORMA Platz 1
10117 Berlin 58256 Ennepetal
Germany Germany
Declaration number Declared product / declared unit
EPD-DOR-20220166-CBA1-EN 1 piece of the product: one (1) dormakaba Kentaur Full-Height Turnstile
(FTS-E02), consisting of the following items:
- drive and control unit
- ground kit
- key for cylinder casing
- floor bearing for Full-height Turnstiles
- cement for Full-height Turnstiles
- maintenance flaps - fastening material - packaging material
This declaration is based on the product category rules: Scope:
Electronic and physical Access Control Systems, 01.08.2021 This EPD is a specific product declaration for the Kentaur Full-Height
(PCR checked and approved by the SVR) Turnstiles (FTS-E02).
The underlying life cycle assessment is based on the entire life cycle of
this specific Kentaur Full-Height Turnstile.
Issue date The products are manufactured at the dormakaba production facility in
Bühl (Germany).
17.10.2022
Green electricity is being used at this production site.
Data represents the year 2022.
Valid to
The owner of the declaration shall be liable for the underlying information
16.10.2027 and evidence; the IBU shall not be liable with respect to manufacturer
information, life cycle assessment data and evidences.
The EPD was created according to the specifications of EN 15804+A2. In
the following, the standard will be simplified as EN 15804.
Verification
The standard EN 15804 serves as the core PCR
Independent verification of the declaration and data according to ISO
14025:2011
internally X externally
Dipl.-Ing. Hans Peters
(Chairman of Institut Bauen und Umwelt e.V.)
Florian Pronold Dr.-Ing. Wolfram Trinius,
(Managing Director Institut Bauen und Umwelt e.V.) (Independent verifier)
1 Environmental Product Declaration - Dormakaba - Kentaur
Product
Product description/Product definition Technical Data
The robust Kentaur Full-Height Turnstiles are especially Following technical data apply for the Kentaur Full-Height
suitable for securing the perimeter of buildings and property. Turnstile (FTS-E02):
Versatile versions enable individual combinations of multiple
Technical data
units to be put together. The end point locking system
Name ValueUnit
developed by dormakaba prevents people from being trapped
in the gates. Column diameter 1300 mm
Portal width 1540 mm
Versatility Total height (without opt. roof) 2270 mm
The Kentaur product series offers a modular design. Two, three
Passage height 2060 mm
and four-winged units with straight or U-shaped bars can be
Passage width 646 mm
combined with each other. The same applies for units with
bicycle doors, integrated doors, an emergency exit function of Power supply 253 VA
resistance class RC2. The roofs fit with any of the single, Standby power consumption 20 VA
multiple or space-saving double units. Protection classes Housing 33 IP
Protection classes Components conducting supply
Minimal power consumption 43 IP
voltage
The low-energy drive consumes little energy.
Kentaur Full-Height Turnstiles include the following
Safe passage components:
The end point locking implemented in Kentaur turnstiles - drive and control unit
prevents people from becoming trapped or jammed. After - ground kit
release the turnstile may be stopped at any time and rotated - key for cylinder casing
backwards as long as it has not yet completed half of its - floor bearing for Full-Height Turnstiles
rotation. - cement for Full-Height Turnstiles
Once the turnstile has completed half of its rotary motion, the - maintenance flaps - fastening material - packaging material
unit can only be exited in the released direction. For the placing
on the market in the European Union/European Free Trade The total weight of all components is 302,95 kg, including
Associaton (EU/EFTA) (with the exception of Switzerland) the packaging (among others wooden pallets) 418,40 kg.
following legal provisions apply:
Product not harmonised in accordance with the CPR but in
• Machinery Directive 2006/42/EC
accordance with other provisions for harmonisation of the EU:
• 2014/30/EU Electromagnetic Compatibility Directive
• 2011/65/EU ROHS2 Directive • Machinery Directive 2006/42/EC
• DIN EN ISO 12100:2011-03 Safety of machinery • 2014/30/EU Electromagnetic Compatibility Directive
• DIN EN 16005: 2013-01 and Amendment 2015-10 • 2011/65/EU ROHS2 Directive
Power operated pedestrian doorsets • DIN EN ISO 12100:2011-03 Safety of machinery
• DIN EN ISO 13849- 1:2016-06 Safety of machinery • DIN EN 16005: 2013-01 and Amendment 2015-10
• DIN EN ISO 13849- 2:2013-02 Safety of machinery Power operated pedestrian doorsets
• DIN EN 60335-2-103: 2016-05 Household and similar • DIN EN ISO 13849- 1:2016-06 Safety of machinery
electrical appliances • DIN EN ISO 13849- 2:2013-02 Safety of machinery
• DIN EN 61000-3-2:2015-03 Electromagnetic • DIN EN 60335-2-103: 2016-05 Household and similar
compatibility (EMC) electrical appliances
• DIN EN 61000-6-2: 2005 and Amendment:2011 • DIN EN 61000-3-2:2015-03 Electromagnetic
Electromagnetic Compatibility (EMC) compatibility (EMC)
• DIN EN 61000-6-3:2007 and A1:2011 Electromagnetic • DIN EN 61000-6-2: 2005 and Amendment:
Compatibility (EMC) 2011 Electromagnetic Compatibility (EMC)
The CE-marking takes into account the proof of conformity with • DIN EN 61000-6-3:2007 and A1:2011 Electromagnetic
the respective harmonized standards based on the legal Compatibility (EMC)
provisions above.
Base materials/Ancillary materials
For the application and use the respective national provisions
For the main Kentaur Full-Height Turnstiles (FTS-E02) product
apply.
components the composition is the following:
Application
For reliabable security at:
• Manufacturing plants
• Company sites
• Airports and ports
• Power plants
• Car parks
• Bicycle stands
• Correctional facilities
• Military installations
• Educational centres
• Stadiums The product includes partial articles which contain substances
• Amusement parks listed in the Candidate List of REACH Regulation
2 Environmental Product Declaration - Dormakaba - Kentaur
1907/2006/EC (date: 10.06.2022) exceeding 0.1 percentage by
mass: no Reference service life
The reference service life amounts to 15 years according to EN
The Candidate List can be found on the ECHA website 16005.
address: https://echa.europa.eu/de/home.
LCA: Calculation rules
The use stage related to the operation of the building includes:
Declared Unit — B6, operational energy use
The declared unit is 1 piece of product: 302,95 kg The potential use of electricity from the grid is declared in
Declared unit module B6.
Name Value Unit
End-of-life stage– Modules C1-C4 and D
Declared unit 1 pce.
The end-of-life stage includes:
Mass (total system excluding packaging) 306.49 kg — C1, de-construction, demolition:
— C2, transport to waste processing;
System boundary — C3, waste processing for reuse, recovery and/or recycling;
Type of EPD: cradle to gate with options, modules C1–C4, and — C4, disposal;
module D (A1–A3 + C + D and additional modules: A4 + A5 + including provision and all transport, provision of all materials,
B6) products and related energy and water use.
Production - Module A1-A3 Module D (Benefits and loads beyond the system boundary)
The product stage includes: includes:
— A1, raw material extraction, processing and mechanical — D, recycling potentials, expressed as net impacts and
treatments, processing of secondary material input (e.g. benefits.
recycling processes),
— A2, transport to the manufacturer,
Geographic Representativeness
— A3, manufacturing and assembly including provision of all
Land or region, in which the declared product system is
materials, products and energy, as well as waste processing up
manufactured, used or handled at the end of the product´s
to the end-of waste state.
lifespan: Germany
Construction stage - Modules A4-A5
The construction process stage includes:
Comparability
— A4, transport to the building site;
Basically, a comparison or an evaluation of EPD data is only
— A5, installation into the building;
possible if all the data sets to be compared were created
including provision of all materials, products and energy, as well
according to EN 15804 and the building context, respectively
as waste processing up to the end-of-waste state or disposal of
the product-specific characteristics of performance, are taken
final residues during the construction process stage.
into account. Background
database: GaBi , SP40.
Use stage - Module B6
LCA: Scenarios and additional technical information
Transport distance is declared for a distance of 100km by truck
Characteristic product properties of biogenic carbon in order to allow scaling to a specific point of installation.
Information on describing the biogenic Carbon Content at
factory gate Installation into the building (A5)
Name ValueUnit Name Value Unit
kg Waste packaging (paper and plastic) kg
Biogenic carbon content in product 0.41
C
Biogenic carbon content in accompanying kg Reference service life
0.37
packaging C Name Value Unit
Note: 1 kg of biogenic carbon is equivalent to 44/12 kg of CO . Life Span according to the manufacturer 15 a
2
Operational energy use (B6)
The use stage is declared for 15 years
The following technical scenario information is required for the
declared modules Name Value Unit
Days per year in use 365 days
Transport to the building site (A4)
On mode per day 1 hours
Name Value Unit
Idle mode per day 23 hours
Litres of fuel (per 1 kg) 0.00276l/100km
On mode power 47 W
Transport distance via medium truck 100 km
Idle mode power 9 W
Capacity utilisation (including empty runs) via
medium truck 55 % Electricity consumption per 1 year 92,71 kWh
End of life (C1-C4)
3 Environmental Product Declaration - Dormakaba - Kentaur
C1: The product dismantling from the building is done manually Material recycling is then assumed for the metals, electronics
without environmental burden. and electromechanics. The plastic components are assumed to
Name Value Unit be incinerated with energy recovery. Minor proportions of
residues arising from the recycling process are landfilled.
Collected separately waste type waste type 306.49 kg
Recycling 252 kg
The region for the End of Life is: Europe.
Energy recovery 3.69 kg
Landfilling 50.8 kg Reuse, recovery and/or recycling potentials (D), relevant
Transport to waste management 50 km scenario information
Collection rate is 100%.
The product is disassembled in a recycling process.
4 Environmental Product Declaration - Dormakaba - Kentaur
LCA: Results
DESCRIPTION OF THE SYSTEM BOUNDARY (X = INCLUDED IN LCA; MND = MODULE OR INDICATOR NOT DECLARED; MNR
= MODULE NOT RELEVANT)
Benefits and
Construction loads beyond
Product stage Use stage End of life stage
process stage the system
boundaries
la ire ta m w a Ry lp p u s tro p s n a rT g n iru tc a fu n a M e h t m o rf tro p s n a rTe tis e h t o t e ta g y lb m e s s A e s U e c n a n e tn ia M ria p e R tn e m e c a lp e R tn e m h s ib ru fe R y g re n e la n o ita re p Oe s u re ta w la n o ita re p Oe s u n o itc u rts n o c -e Dn o itilo m e d tro p s n a rT g n is s e c o rp e ts a W la s o p s iD -e s u e R-y re v o c e R-g n ilc y c e Rla itn e to p
A1 A2 A3 A4 A5 B1 B2 B3 B4 B5 B6 B7 C1 C2 C3 C4 D
X X X X X MND X MNR MNR MNR X MND X X X X X
RESULTS OF THE LCA - ENVIRONMENTAL IMPACT according to EN 15804+A2: 1 piece Kentaur Full-Height Turnstiles
Parameter Unit A1-A3 A4 A5 B2 B6 C1 C2 C3 C4 D
GWP-total kg CO 2 eq 6.79E+02 2.68E+00 3.07E+00 0 5.62E+02 0 1.34E+00 1.14E+01 7.75E-01 -2.9E+02
GWP-fossil kg CO 2 eq 6.81E+02 2.56E+00 1.69E+00 0 5.6E+02 0 1.28E+00 9.41E+00 7.7E-01 -2.91E+02
GWP-
biogenic kg CO 2 eq -3.45E+00 1.18E-01 1.38E+00 0 1.87E+00 0 5.9E-02 1.99E+00 3E-03 1.11E+00
GWP-luluc kg CO 2 eq 1.06E+00 6.1E-05 1.17E-04 0 8.11E-01 0 3.05E-05 5.5E-04 2E-03 -4.95E-01
ODP kg CFC11 eq 2.87E-10 2.71E-16 1.09E-15 0 1.23E-11 0 1.35E-16 4.98E-15 2.86E-15 -3.34E-10
AP mol H+ eq 3.09E+00 3E-03 6.91E-04 0 1.24E+00 0 1E-03 2E-03 6E-03 -1.28E+00
EP-
kg P eq 1.16E-03 5.48E-07 1.83E-07 0 1E-03 0 2.74E-07 7.91E-07 1.32E-06 -2.4E-04
freshwater
EP-marine kg N eq 4.43E-01 8.16E-04 2.1E-04 0 2.75E-01 0 4.08E-04 4.71E-04 1E-03 -1.95E-01
EP-terrestrial mol N eq 4.79E+00 9E-03 3E-03 0 2.88E+00 0 5E-03 9E-03 1.6E-02 -2.12E+00
kg NMVOC
POCP 1.38E+00 2E-03 5.64E-04 0 7.52E-01 0 1E-03 1E-03 4E-03 -5.82E-01
eq
ADPE kg Sb eq 3.1E-02 7.68E-08 1.55E-08 0 1.62E-04 0 3.84E-08 6.88E-08 6.92E-08 -8E-03
ADPF MJ 8.83E+03 3.63E+01 1.21E+00 0 9.84E+03 0 1.82E+01 4.78E+00 1.01E+01 -3.66E+03
m3 world eq
WDP 1.95E+02 5E-03 3.45E-01 0 1.22E+02 0 3E-03 1.17E+00 8.1E-02 -1.03E+02
deprived
GWP = Global warming potential; ODP = Depletion potential of the stratospheric ozone layer; AP = Acidification potential of land and water; EP =
Eutrophication potential; POCP = Formation potential of tropospheric ozone photochemical oxidants; ADPE = Abiotic depletion potential for non-fossil
resources; ADPF = Abiotic depletion potential for fossil resources; WDP = Water (user) deprivation potential)
RESULTS OF THE LCA - INDICATORS TO DESCRIBE RESOURCE USE according to EN 15804+A2: 1 piece Kentaur Full-Height
Turnstiles
Parameter Unit A1-A3 A4 A5 B2 B6 C1 C2 C3 C4 D
PERE MJ 2.57E+03 1.15E-01 1.23E+01 0 4.36E+03 0 5.7E-02 1.45E+01 1.32E+00 -9.33E+02
PERM MJ 2.53E+01 0 -1.2E+01 0 0 0 0 -1.33E+01 0 0
PERT MJ 2.6E+03 1.15E-01 2.81E-01 0 4.36E+03 0 5.7E-02 1.21E+00 1.32E+00 -9.33E+02
PENRE MJ 8.65E+03 3.64E+01 2.92E+01 0 9.84E+03 0 1.82E+01 1.6E+02 1.01E+01 -3.66E+03
PENRM MJ 1.83E+02 0 -2.8E+01 0 0 0 0 -1.55E+02 0 0
PENRT MJ 8.84E+03 3.64E+01 1.21E+00 0 9.84E+03 0 1.82E+01 4.79E+00 1.01E+01 -3.66E+03
SM kg 2.28E+02 0 0 0 0 0 0 0 0 0
RSF MJ 0 0 0 0 0 0 0 0 0 0
NRSF MJ 0 0 0 0 0 0 0 0 0 0
FW m3 7.79E+00 2.06E-04 8E-03 0 5.04E+00 0 1.03E-04 2.8E-02 3E-03 -4.48E+00
PERE = Use of renewable primary energy excluding renewable primary energy resources used as raw materials; PERM = Use of renewable primary
energy resources used as raw materials; PERT = Total use of renewable primary energy resources; PENRE = Use of non-renewable primary energy
excluding non-renewable primary energy resources used as raw materials; PENRM = Use of non-renewable primary energy resources used as raw
materials; PENRT = Total use of non-renewable primary energy resources; SM = Use of secondary material; RSF = Use of renewable secondary fuels;
NRSF = Use of non-renewable secondary fuels; FW = Use of net fresh water
RESULTS OF THE LCA – WASTE CATEGORIES AND OUTPUT FLOWS according to EN 15804+A2:
1 piece Kentaur Full-Height Turnstiles
Parameter Unit A1-A3 A4 A5 B2 B6 C1 C2 C3 C4 D
HWD kg 3.22E-05 3.53E-09 3.58E-09 0 4.07E-06 0 1.76E-09 1.69E-08 1.54E-07 -1.59E-06
NHWD kg 6.3E+01 4E-03 2.16E-01 0 6.98E+00 0 2E-03 9.89E-01 5.08E+01 -3.53E+01
RWD kg 3.01E-01 3.9E-05 5.2E-05 0 1.49E+00 0 1.95E-05 1.86E-04 1.15E-04 -8.7E-02
CRU kg 0 0 0 0 0 0 0 0 0 0
MFR kg 0 0 0 0 0 0 0 2.51E+02 0 0
MER kg 0 0 0 0 0 0 0 0 0 0
EEE MJ 0 0 5.21E+00 0 0 0 0 0 0 0
5 Environmental Product Declaration - Dormakaba - Kentaur
EET MJ 0 0 1.09E+01 0 0 0 0 0 0 0
HWD = Hazardous waste disposed; NHWD = Non-hazardous waste disposed; RWD = Radioactive waste disposed; CRU = Components for re-use;
MFR = Materials for recycling; MER = Materials for energy recovery; EEE = Exported electrical energy; EET = Exported thermal energy
RESULTS OF THE LCA – additional impact categories according to EN 15804+A2-optional:
1 piece Kentaur Full-Height Turnstiles
Parameter Unit A1-A3 A4 A5 B2 B6 C1 C2 C3 C4 D
Disease
PM 4.85E-05 1.35E-08 5.95E-09 0 1.04E-05 0 6.74E-09 2.28E-08 6.84E-08 -2.5E-05
incidence
IR kBq U235 eq 4.01E+01 6E-03 6E-03 0 2.45E+02 0 3E-03 1.8E-02 1.2E-02 -1.63E+01
ETP-fw CTUe 3.81E+03 2.58E+01 5E-01 0 4.21E+03 0 1.29E+01 1.82E+00 5.78E+00 -1.83E+03
HTP-c CTUh 7.97E-05 4.84E-10 3.61E-11 0 1.16E-07 0 2.42E-10 1.54E-10 8.56E-10 -5.27E-07
HTP-nc CTUh 1.23E-05 2.07E-08 3.01E-09 0 4.28E-06 0 1.04E-08 1.48E-08 9.43E-08 -1.56E-06
SQP SQP 2.13E+03 9.3E-02 3.48E-01 0 3.13E+03 0 4.7E-02 1.42E+00 2.11E+00 -4.66E+02
PM = Potential incidence of disease due to PM emissions; IR = Potential Human exposure efficiency relative to U235; ETP-fw = Potential comparative
Toxic Unit for ecosystems; HTP-c = Potential comparative Toxic Unit for humans (cancerogenic); HTP-nc = Potential comparative Toxic Unit for humans
(not cancerogenic); SQP = Potential soil quality index
Disclaimer 1 – for the indicator 'Potential Human exposure efficiency relative to U235'.This impact category deals mainly with the
eventual impact of low-dose ionizing radiation on human health of the nuclear fuel cycle. It does not consider effects due to possible
nuclear accidents, occupational exposure or radioactive waste disposal in underground facilities.
Potential ionizing radiation from the soil, radon and from some construction materials is also not measured by this indicator.
Disclaimer 2 – for the indicators 'abiotic depletion potential for non-fossil resources', 'abiotic depletion potential for fossil resources',
'water (user) deprivation potential, deprivation-weighted water consumption', 'potential comparative toxic unit for ecosystems', 'potential
comparative toxic unit for humans – cancerogenic', 'Potential comparative toxic unit for humans - not cancerogenic', 'potential soil
quality index'.
The results of this environmental impact indicator shall be used with care as the uncertainties on these results are high as there is
limited experience with the indicator.
References
DIN EN 16005 DIN EN ISO 14025:2011-10,
DIN EN 16005: 201301 and Amendment 2015-10 Power Environmental labels and declarations — Type III
operated pedestrian doorsets environmental declarations —
Principles and procedures.
DIN EN 60335-2
DIN EN 603352103: 201605 Household and similar electrical Electromagnetic Compatibility Directive 2014/30/EU
appliances DIRECTIVE 2014/30/EU OF THE EUROPEAN PARLIAMENT
AND OF THE COUNCILof 26 February 2014on the
DIN EN 61000-3-2 harmonisation of the laws of the Member States relating to
DIN EN 6100032: 201503 Electromagnetic electromagnetic compatibility
compatibility (EMC) European Waste Catalogue (EWC)
COMMISSION DECISION of 18 December 2014 amending
DIN EN 61000-6-2 Decision 2000/532/EC on the list of waste pursuant to Directive
DIN EN 6100062: 2005 and Amendment:2011 Electromagnetic 2008/98/EC of the European Parliament and of the Council
Compatibility (EMC)
Machinery Directive 2006/42/EC
DIN EN 61000-6-3 DIRECTIVE 2006/42/EC OF THE EUROPEAN PARLIAMENT
DIN EN 6100063: 2007 and A1:2011 Electromagnetic AND OF THE COUNCILof 17 May 2006on machinery, and
Compatibility (EMC) amending Directive 95/16/EC
DIN EN ISO 12100 REACH
DIN EN ISO 12100:201103 Safety of machinery Regulation (EC) No 1907/2006 of the European Parliament and
of the Council on the Registration, Evaluation, Authorisation
DIN EN ISO 13849- 1 and Restriction of Chemicals (REACH) ROHS2 Directive
DIN EN ISO 138491: 201606 Safety of machinery Directive 2011/65/EU of the European Parliament and of the
Council of 8 June 2011 on the restriction of the use of certain
DIN EN ISO 13849- 2 hazardous substances in electrical and electronic equipment
DIN EN ISO 138492: 201302 Safety of machinery
Further References
EN 15804
EN 15804 + A2:2019, Sustainability of construction works — IBU 2021
Environmental Product Declarations — Core rules for the General Instructions for the EPD programme of Institut Bauen
product category of construction products. und Umwelt e.V. Version 2.0, Berlin: Institut
Bauen und Umwelt e.V., 2021
ISO 9001 www.ibu-epd.com
ISO 9001:201509 Quality management systems Requirements
GaBi ts software
ISO 14025 Sphera Solutions GmbH Gabi Software System and Database
6 Environmental Product Declaration - Dormakaba - Kentaur
for Life Cycle Engineering 19922020 Version 10.0.0.71
University of Stuttgart Leinfelden-Echterdingen PCR Part A
PCR – Part A: Calculation Rules for the Life Cycle Assessment
GaBi ts documentation and Requirements on the Project Report according to EN
GaBi life cycle inventory data documentation 15804+A2:2019, Version 1.0, Institut Bauen und Umwelt e.V.,
(https://www.gabisoftware. www.ibu-epd.com.
com/support/gabi/gabidatabase[1]2020lcidocumentati on/).
PCR Part B
LCA-tool dormakaba PCR – Part B: Requirements on the EPD for electronic and
LCA tool, ESC (Entrance System Control) Tool No.: IBU-DOR- physical Access Control Systems, version 1.2, Institut Bauen
202109-LT1-EN und Umwelt e.V., www.ibuepd.
Developed by Sphera Solutions GmbH. com, 2019.
7 Environmental Product Declaration - Dormakaba - Kentaur
Publisher
Institut Bauen und Umwelt e.V. +49 (0)30 3087748- 0
Hegelplatz 1 info@ibu-epd.com
10117 Berlin www.ibu-epd.com
Germany
Programme holder
Institut Bauen und Umwelt e.V. +49 (0)30 3087748- 0
Hegelplatz 1 info@ibu-epd.com
10117 Berlin www.ibu-epd.com
Germany
Author of the Life Cycle Assessment
Sphera Solutions GmbH +49 711 341817-0
Hauptstraße 111- 113 info@sphera.com
70771 Leinfelden-Echterdingen www.sphera.com
Germany
Owner of the Declaration
dormakaba International Holding GmbH +49 2333 793-0
DORMA Platz 1 info.de@dormakaba.com
58256 Ennepetal www.dormakaba.com
Germany
8 Environmental Product Declaration - Dormakaba - Kentaur
