ENVIRONMENTAL PRODUCT DECLARATION
as per ISO 14025 and EN 15804+A2
Owner of the Declaration dormakaba International Holding GmbH
Publisher Institut Bauen und Umwelt e.V. (IBU)
Programme holder Institut Bauen und Umwelt e.V. (IBU)
Declaration number EPD-DOR-20230070-CBA2-EN
Issue date 30/06/2023
Valid to 29/06/2028
Folding door system FFT FLEX Green
dormakaba
www.ibu-epd.com | https://epd-online.com
General Information
dormakaba Folding door system FFT FLEX Green
Programme holder Owner of the declaration
IBU – Institut Bauen und Umwelt e.V. dormakaba International Holding GmbH
Hegelplatz 1 DORMA Platz 1
10117 Berlin 58256 Ennepetal
Germany Germany
Declaration number Declared product / declared unit
EPD-DOR-20230070-CBA2-EN 1 piece of the product: Folding door system FFT FLEX Green, consisting
of the following items:
• ES 200 FFT drive unit
• Pairs of folding panels
• Hold-open columns
• Floor rail
• Product packaging
This declaration is based on the product category rules: Scope:
Automatic doors, automatic gates, and revolving door systems, This Environmental Product Declaration refers to a specific folding door
01/08/2021 system manufactured by dormakaba. The production site is located in
(PCR checked and approved by the SVR) Ennepetal (Germany). Green electricity is being used at this production
site.
Issue date Data represents the year 2022.
The owner of the declaration shall be liable for the underlying information
30/06/2023
and evidence; the IBU shall not be liable with respect to manufacturer
information, life cycle assessment data and evidences.
Valid to
The EPD was created according to the specifications of EN 15804+A2. In
29/06/2028 the following, the standard will be simplified as EN 15804.
Verification
The standard EN 15804 serves as the core PCR
Independent verification of the declaration and data according to ISO
14025:2011
internally X externally
Dipl.-Ing. Hans Peters
(Chairman of Institut Bauen und Umwelt e.V.)
Florian Pronold Dr.-Ing. Wolfram Trinius,
(Managing Director Institut Bauen und Umwelt e.V.) (Independent verifier)
1 Environmental-Product Declaration - dormakaba - Folding door system FFT FLEX Green
Product
The automatic folding door has the following technical
Product description/Product definition properties:
The FFT FLEX Green is an automatic folding door with
Name Value Unit
thermally separated, particularly slim profiles and a silent,
Opening and closing force maximum 150 N
dynamic drive system. It is particularly suitable where space is
restricted. It permits opening widths of up to 2.4 metres and Opening speed incremental adjustment 10-75 cm/s
achieves therefore a maximum escape route width. Maximum Closing speed incrementally variable 10-50 cm/s
heights of up to 2.5 metres are possible. Hold-open time 0-180 s
Installed load, frequency 230 V
The FFT FLEX Green folding door avails of highly efficient
Power consumption 250 W
thermal separation with very good thermal transmittance values
(UD values) ranging from 1.7 to max. 2.4 (thermal coefficient) Type of protection 20 IP
which can be calculated individually for each door system. In Clear opening width maximum 900-2400 mm
combination with ISO glass, the FFT FLEX Green ensures Panel pair weight maximum 90 kg
good thermal insulation of external doors.
Clear passage height 2100-2500 mm
Double glazing 28 ISO
For the use and application of the product the representative
national provisions apply. For the FFT FLEX Green the Performance data of the product with respect to its
standards which can be applied are the following: characteristics in accordance with the relevant technical
provision which can be applied are mentioned above.
• EN 18650-1
• EN 18650-2
• EN 16005 Base materials/Ancillary materials
• EN 60335-1
The major material composition including the packaging of the
• ISO 13849-1
product is listed below.
• 2011/65/EU ROHS3 Directive
Name Value Unit
• Machinery Directive 2006/42/EC
Glass 42 %
The CE marking takes into account the proof of conformity with Aluminium 27 %
the respective harmonized standards based on the legal Steel 19 %
provisions above.
Plastic 6 %
Plastic packaging 4 %
Application Electronics 1 %
The FFT FLEX Green folding door is used when a wide an Zinc 1 %
opening width is to be achieved despite low wall opening
The FFT FLEX Green includes partial articles which contain
dimensions. It is suitable for both external and internal doors in
substances listed in the Candidate List of REACH Regulation
narrow passageways, barrier-free access points in public
1907/2006/EC (date: 17.01.2023) exceeding 0.1 percentage by
buildings as well as escape routes and emergency exits. While
mass: yes
opening, the door panel is simultaneously folded and
automatically moved to the side.
• Lead (Pb): 7439-92-1 (CAS-No.) is used in some of the
alloys. The concentration of lead in each individual alloy
Bi-parting opening
does not exceed 4.0%
Both pairs of door panels are synchronously swivelled
(by mass).
to the side and in opposing directions while opening,
thereby permitting a maximum opening width of 2.4 metres.
The Candidate List can be found on the ECHA website
address: https:echa.europa.eu/de/home.
Unilateral opening
For smaller applications: the FFT FLEX Green folding Reference service life
door comprising a single pair of panels permits a
The reference service life of the product amounts to 10 years
maximum opening width of 1.2 metres.
and depends on the application and frequency of use. Regular
maintenance is advised to ensure the life expectancy of 10
Technical Data
years. For repairs and renewals, suitable spare parts are
available. The product is tested and certified to EN 16005,
Technical data meaning they are designed to withstand a minimum of
1.000.000 cycles.
LCA: Calculation rules
For IBU core EPDs (where clause 3.6 is part of the EPD): for
Declared Unit average EPDs, an estimate of the robustness of the LCA
The declared unit is 1 piece of the product: FFT FLEX Green values must be made, e.g. concerning the variability of the
Name Value Unit production process, geographical representativeness and the
Declared unit 1 pce. influence of background data and preliminary products
compared to the environmental impacts caused by the actual
Mass of the entire system 223.03 kg
production.
2 Environmental-Product Declaration - dormakaba - Folding door system FFT FLEX Green
— B6, operational energy use
System boundary
The type of EPD is: cradle to gate with options, End-of-life stage– Modules C1-C4 and D
modules C1–C4, and module D (A1–A3 + C + D and The end-of-life stage includes:
additional modules: A4 + A5 + B6) — C1, deconstruction, demolition:
— C2, transport to waste processing;
Production - Module A1-A3 — C3, waste processing for reuse, recovery and/or
The product stage includes: recycling;
— A1, raw material extraction, processing and — C4, disposal;
mechanical treatments, processing of secondary including provision and all transport, provision of all
material input (e.g. recycling processes), materials, products and related energy and water use.
— A2, transport to the manufacturer, Module D (Benefits and loads beyond the system
— A3, manufacturing and assembly including provision boundary) includes:
of all materials, products and energy, as well as waste — D, recycling potentials, expressed as net impacts
processing up to the end-of waste state. and benefits.
Construction stage - Modules A4-A5 Geographic Representativeness
The construction process stage includes: Land or region, in which the declared product system is
— A4, transport to the building site; manufactured, used or handled at the end of the product´s
— A5, installation into the building; lifespan: Global
including provision of all materials, products and
energy, as well as waste processing up to the end-of
Comparability
waste state or disposal of final residues during the
construction process stage. Basically, a comparison or an evaluation of EPD data is only
possible if all the data sets to be compared were created
Use stage - Module B6 according to EN 15804 and the building context, respectively
The use stage related to the operation of the building the product-specific characteristics of performance, are taken
includes: into account. Background database: GaBi, SP40
LCA: Scenarios and additional technical information
Characteristic product properties biogenic carbon
Reference service life
The biogenic carbon content quantifies the amount of biogenic
carbon in a construction product leaving the factory gate, and it Name Value Unit
shall be separately declared for the product and for any Life Span according to the manufacturer 10 a
accompanying packaging.
If the total mass of biogenic carbon containing materials is less Operational energy use (B6)
than 5 % of the total mass of the product and accompanying Name Value Unit
packaging, the declaration of biogenic carbon content may be Electricity consumption for 1 year 224.65 kWh
omitted. The mass of packaging containing biogenic carbon
Days per year in use 365 days
shall always be declared.
Active mode per day 1,80 h
Note: 1 kg of biogenic carbon is equivalent to 44/12 kg of CO2. Idle mode per day 22,20 h
Active mode power 16,33 W
Information on describing the biogenic carbon content at Idle mode power 26,40 W
factory gate
End of life (C1-C4)
Name ValueUnit
C1: The product expansion depends on the building. The
kg
Biogenic carbon content in product 0.05 product share is so low that no environmental burden is
C
assumed.
Biogenic carbon content in accompanying kg C2: Transport to waste management 50 km.
0.08
packaging C
Name Value Unit
Collected separately waste type 214 kg
Transport to the building site (A4) Recycling 106 kg
Name Value Unit Energy recovery 13 kg
Litres of fuel (per 1kg) 0.00276 l/100km Landfilling 94.8 kg
Capacity utilisation (including empty runs) 55 %
Transport distance via medium truck 100 km The product is disassembled in a recycling process. Material
recycling is then assumed for the metals and electronics. The
The product is transported via truck. The main distribution
plastic components are assumed to be incinerated with energy
region is Europe. In order to allow scaling to a specific point of
recovery. Electromechanics and minor proportions of residues
installation 100 km are declared.
arising from the recycling process are landfilled.
Region for the End of Life is: Global.
Installation into the building (A5)
Name Value Unit
Reuse, recovery and/or recycling potentials (D), relevant
Waste packaging (paper and plastic) 9,198 kg scenario information
3 Environmental-Product Declaration - dormakaba - Folding door system FFT FLEX Green
Name Value Unit The collection rate is 100%.
Recycling 100 %
4 Environmental-Product Declaration - dormakaba - Folding door system FFT FLEX Green
LCA: Results
DESCRIPTION OF THE SYSTEM BOUNDARY (X = INCLUDED IN LCA; ND = MODULE OR INDICATOR NOT DECLARED; MNR =
MODULE NOT RELEVANT)
Benefits and
Construction loads beyond
Product stage Use stage End of life stage
process stage the system
boundaries
la ire ta m w a Ry lp p u s tro p s n a rT g n iru tc a fu n a M e h t m o rf tro p s n a rTe tis e h t o t e ta g y lb m e s s A e s U e c n a n e tn ia M ria p e R tn e m e c a lp e R tn e m h s ib ru fe R y g re n e la n o ita re p Oe s u re ta w la n o ita re p Oe s u n o itc u rts n o c -e Dn o itilo m e d tro p s n a rT g n is s e c o rp e ts a W la s o p s iD -e s u e R-y re v o c e R-g n ilc y c e Rla itn e to p
A1 A2 A3 A4 A5 B1 B2 B3 B4 B5 B6 B7 C1 C2 C3 C4 D
X X X X X MND X MNR MNR MNR X MND X X X X X
RESULTS OF THE LCA - ENVIRONMENTAL IMPACT according to EN 15804+A2: 1 piece FFT FLEX Green
Parameter Unit A1-A3 A4 A5 B2 B6 C1 C2 C3 C4 D
GWP-total kg CO 2 eq 5.05E+02 1.95E+00 2.32E+01 0 0 0 9.34E-01 3.35E+01 1.45E+00 -1.61E+02
GWP-fossil kg CO 2 eq 5.04E+02 1.87E+00 2.29E+01 0 0 0 8.93E-01 3.33E+01 1.44E+00 -1.6E+02
GWP-
biogenic kg CO 2 eq 8.28E-01 8.6E-02 3.17E-01 0 0 0 4.1E-02 2.23E-01 5E-03 -1.52E-01
GWP-luluc kg CO 2 eq 3.15E-01 4.44E-05 1E-03 0 0 0 2.13E-05 2E-03 4E-03 -1.04E-01
ODP kg CFC11 eq 1.67E-09 1.97E-16 1.16E-14 0 0 0 9.43E-17 1.68E-14 5.33E-15 -6.06E-10
AP mol H+ eq 2.58E+00 2E-03 4E-03 0 0 0 8.94E-04 6E-03 1E-02 -5.49E-01
EP-
kg P eq 5.68E-04 3.99E-07 1.85E-06 0 0 0 1.91E-07 2.68E-06 2.47E-06 -1.26E-04
freshwater
EP-marine kg N eq 5.41E-01 5.94E-04 9.34E-04 0 0 0 2.84E-04 1E-03 3E-03 -8.3E-02
EP-terrestrial mol N eq 6.03E+00 7E-03 1.9E-02 0 0 0 3E-03 2.7E-02 2.9E-02 -8.9E-01
kg NMVOC
POCP 1.4E+00 2E-03 3E-03 0 0 0 8.04E-04 4E-03 8E-03 -2.62E-01
eq
ADPE kg Sb eq 1.3E-02 5.59E-08 1.59E-07 0 0 0 2.68E-08 2.31E-07 1.29E-07 -4E-03
ADPF MJ 7.26E+03 2.64E+01 1.07E+01 0 0 0 1.27E+01 1.55E+01 1.89E+01 -2.19E+03
m3 world eq
WDP 4.89E+01 4E-03 2.38E+00 0 0 0 2E-03 3.43E+00 1.51E-01 -2.33E+01
deprived
GWP = Global warming potential; ODP = Depletion potential of the stratospheric ozone layer; AP = Acidification potential of land and water; EP =
Eutrophication potential; POCP = Formation potential of tropospheric ozone photochemical oxidants; ADPE = Abiotic depletion potential for non-fossil
resources; ADPF = Abiotic depletion potential for fossil resources; WDP = Water (user) deprivation potential)
RESULTS OF THE LCA - INDICATORS TO DESCRIBE RESOURCE USE according to EN 15804+A2: 1 piece FFT FLEX Green
Parameter Unit A1-A3 A4 A5 B2 B6 C1 C2 C3 C4 D
PERE MJ 1.28E+03 8.3E-02 5.35E+00 0 0 0 4E-02 5.51E+00 2.47E+00 -7.01E+02
PERM MJ 4.06E+00 0 -2.57E+00 0 0 0 0 -1.49E+00 0 0
PERT MJ 1.28E+03 8.3E-02 2.77E+00 0 0 0 4E-02 4.02E+00 2.47E+00 -7.01E+02
PENRE MJ 6.62E+03 2.65E+01 3.98E+02 0 0 0 1.27E+01 2.68E+02 1.89E+01 -2.19E+03
PENRM MJ 6.39E+02 0 -3.87E+02 0 0 0 0 -2.52E+02 0 0
PENRT MJ 7.26E+03 2.65E+01 1.07E+01 0 0 0 1.27E+01 1.55E+01 1.89E+01 -2.19E+03
SM kg 7.83E+01 0 0 0 0 0 0 0 0 0
RSF MJ 0 0 0 0 0 0 0 0 0 0
NRSF MJ 0 0 0 0 0 0 0 0 0 0
FW m3 2.95E+00 1.5E-04 5.7E-02 0 0 0 7.16E-05 8.2E-02 5E-03 -1.66E+00
PERE = Use of renewable primary energy excluding renewable primary energy resources used as raw materials; PERM = Use of renewable primary
energy resources used as raw materials; PERT = Total use of renewable primary energy resources; PENRE = Use of non-renewable primary energy
excluding non-renewable primary energy resources used as raw materials; PENRM = Use of non-renewable primary energy resources used as raw
materials; PENRT = Total use of non-renewable primary energy resources; SM = Use of secondary material; RSF = Use of renewable secondary fuels;
NRSF = Use of non-renewable secondary fuels; FW = Use of net fresh water
RESULTS OF THE LCA – WASTE CATEGORIES AND OUTPUT FLOWS according to EN 15804+A2:
1 piece FFT FLEX Green
Parameter Unit A1-A3 A4 A5 B2 B6 C1 C2 C3 C4 D
HWD kg 2.35E-05 2.57E-09 4.05E-08 0 0 0 1.23E-09 5.89E-08 2.88E-07 -2.29E-05
NHWD kg 5.94E+01 3E-03 2.38E+00 0 0 0 1E-03 3.46E+00 9.49E+01 -2.2E+01
RWD kg 2.07E-01 2.84E-05 3.98E-04 0 0 0 1.36E-05 5.76E-04 2.15E-04 -1.58E-01
CRU kg 0 0 0 0 0 0 0 0 0 0
MFR kg 0 0 0 0 0 0 0 5.65E+01 0 0
MER kg 0 0 0 0 0 0 0 0 0 0
EEE MJ 0 0 4.28E+01 0 0 0 0 6.2E+01 0 0
5 Environmental-Product Declaration - dormakaba - Folding door system FFT FLEX Green
EET MJ 0 0 9.81E+01 0 0 0 0 1.42E+02 0 0
HWD = Hazardous waste disposed; NHWD = Non-hazardous waste disposed; RWD = Radioactive waste disposed; CRU = Components for re-use;
MFR = Materials for recycling; MER = Materials for energy recovery; EEE = Exported electrical energy; EET = Exported thermal energy
RESULTS OF THE LCA – additional impact categories according to EN 15804+A2-optional:
1 piece FFT FLEX Green
Parameter Unit A1-A3 A4 A5 B2 B6 C1 C2 C3 C4 D
Disease
PM 2.25E-05 9.81E-09 5.23E-08 0 0 0 4.7E-09 7.58E-08 1.28E-07 -9.14E-06
incidence
IR kBq U235 eq 3.26E+01 4E-03 3.6E-02 0 0 0 2E-03 5.2E-02 2.2E-02 -2.99E+01
ETP-fw CTUe 5.35E+03 1.87E+01 4.02E+00 0 0 0 8.98E+00 5.81E+00 1.08E+01 -7.63E+02
HTP-c CTUh 1.9E-05 3.53E-10 3.48E-10 0 0 0 1.69E-10 5.03E-10 1.6E-09 -7.25E-08
HTP-nc CTUh 6.75E-06 1.51E-08 3.51E-08 0 0 0 7.22E-09 5.08E-08 1.76E-07 1.64E-06
SQP SQP 7.19E+02 6.8E-02 3.2E+00 0 0 0 3.3E-02 4.64E+00 3.93E+00 -1.58E+02
PM = Potential incidence of disease due to PM emissions; IR = Potential Human exposure efficiency relative to U235; ETP-fw = Potential comparative
Toxic Unit for ecosystems; HTP-c = Potential comparative Toxic Unit for humans (cancerogenic); HTP-nc = Potential comparative Toxic Unit for humans
(not cancerogenic); SQP = Potential soil quality index
Disclaimer 1 – for the indicator “Potential Human exposure efficiency relative to U235”. This impact category deals mainly with the
eventual impact of low-dose ionizing radiation on human health of the nuclear fuel cycle. It does not consider effects due to possible
nuclear accidents, occupational exposure nor due to radioactive waste disposal in underground facilities. Potential ionizing radiation
from the soil, from radon and from some construction materials is also not measured by this indicator.
Disclaimer 2 – for the indicators “abiotic depletion potential for non-fossil resources”, “abiotic depletion potential for fossil resources”,
“water (user) deprivation potential, deprivation-weighted water consumption”, “potential comparative toxic unit for ecosystems”,
“potential comparative toxic unit for humans – cancerogenic”, “Potential comparative toxic unit for humans - not cancerogenic”,
“potential soil quality index”. The results of this environmental impact indicator shall be used with care as the uncertainties on these
results are high or as there is limited experienced with the indicator.
This EPD was created using a software tool.
References
EN 18650 Machinery Directive
EN 18650-1:2010, Powered pedestrian doors Part 1: Directive 2006/42/EC of the European Parliament and
Product requirements and test methods of the Council on machinery, and amending Directive 95/16/EC
EN 18650 Further References
EN 18650-2:2010, Powered pedestrian doors Part 2:
Safety at powered pedestrian doors IBU 2021
General Instructions for the EPD programme of Institut
EN 16005 Bauen und Umwelt e.V. Version 2.0, Berlin: Institut
EN 16005: 2013-01, Power operated pedestrian Bauen und Umwelt e.V., 2021. www.ibu-epd.com
doorsets - Safety in use Requirements and test methods
GaBi
EN 60335 Sphera Solutions GmbH
EN 60335-1, 2103:2020-08, Household and Gabi Software System and Database for Life Cycle
similar electrical appliances - Safety - Part 1: General Engineering 1992-2020
requirements Version 10.0.0.71
University of Stuttgart
EN 61000 Leinfelden Echterdingen
EN 61000-1-2: 2017-07, Electromagnetic
compatibility (EMC) Part 1-2: General - Methodology GaBi ts documentation
for the achievement of functional safety of electrical GaBi life cycle inventory data documentation
and electronic systems including equipment with (https://www.gabisoftware.
regard to electromagnetic phenomena com/support/gabi/gabidatabase
2020lcidocumentation/)
ISO 13849
DIN EN ISO 13849-1:2021-08, Safety of machinery - LCA-tool dormakaba
Safety-related parts of control systems - Part 1: LCA tool, ENS doors
General principles for design Tool No.: IBU-DOR-202108-LT1-EN
Developed by Sphera Solutions GmbH
REACH
Registration, Evaluation, Authorisation and Restriction PCR Part A
of Chemicals (REACH), Regulation (EC) No 1907/2006 PCR – Part A: Calculation Rules for the Life Cycle
Assessment and Requirements on the Project Report
2011/65/EU ROHS3 Directive according to EN 15804+A2:2019, Version 1.0, Institut
Directive 2011/65/EU of the European Parliament and of the Bauen und Umwelt e.V., www.ibu-epd.com.
Council of 8 June 2011 on the restriction of the use of certain
hazardous substances in electrical and electronic equipment PCR Part B
PCR – Part B: Requirements on the EPD for Building
6 Environmental-Product Declaration - dormakaba - Folding door system FFT FLEX Green
Hardware product, version 1.2, Institut Bauen und in the EPD do not need to be listed here again.
Umwelt e.V., www.ibu-epd.com, 2020 The current version of PCR Part A and PCR Part B of the PCR
The literature referred to in the Environmental Product document on which they are based must be referenced.
Declaration must be listed in full.Standards already fully quoted
7 Environmental-Product Declaration - dormakaba - Folding door system FFT FLEX Green
Publisher
Institut Bauen und Umwelt e.V. +49 (0)30 3087748- 0
Hegelplatz 1 info@ibu-epd.com
10117 Berlin www.ibu-epd.com
Germany
Programme holder
Institut Bauen und Umwelt e.V. +49 (0)30 3087748- 0
Hegelplatz 1 info@ibu-epd.com
10117 Berlin www.ibu-epd.com
Germany
Author of the Life Cycle Assessment
dormakaba International Holding GmbH +49 2333 793-0
DORMA Platz 1 info.de@dormakaba.com
58256 Ennepetal www.dormakaba.com
Germany
Owner of the Declaration
dormakaba International Holding GmbH +49 2333 793-0
DORMA Platz 1 info.de@dormakaba.com
58256 Ennepetal www.dormakaba.com
Germany
8 Environmental-Product Declaration - dormakaba - Folding door system FFT FLEX Green
