ENVIRONMENTAL PRODUCT DECLARATION
as per ISO 14025 and EN 15804+A2
Owner of the Declaration Armacell International S.A.
Programme holder Institut Bauen und Umwelt e.V. (IBU)
Publisher Institut Bauen und Umwelt e.V. (IBU)
Declaration number EPD-ARM-20220037-IBB1-EN
Issue date 22.03.2022
Valid to 21.03.2027
NH/ArmaFlex Smart insulation for building equipment and
industrial installations
Armacell GmbH
www.ibu-epd.com | https://epd-online.com
Umwelt Produktdeklaration Name des Herstellers – Name des Produkts
1. General Information
Armacell GmbH NH/ArmaFlex Smart
Programme holder Owner of the declaration
IBU – Institut Bauen und Umwelt e.V. Armacell International S.A.
Panoramastr. 1 Robert-Bosch-Str. 10
10178 Berlin 48153 Münster - Germany
Germany
Declaration number Declared product / declared unit
EPD-ARM-20220037-IBB1-EN 1m³ insulation material NH/ArmaFlex Smart
This declaration is based on the product Scope:
category rules: Product line NH/ArmaFlex Smart
Insulating materials made of foam plastics, 01.2019 Insulation material for industrial and building
(PCR checked and approved by the SVR) installations vulcanized in tubes and sheets.
This declaration is an Environmental Product
Issue date Declaration according to ISO 14025 describing the
22.03.2022 specific environmental performance of the product
produced in Germany.
Valid to
21.03.2027 As the installation of the product is not restricted to
countries where the products have been produced the
validity of this EPD is considered at least EU wide.
The owner of the declaration shall be liable for the
underlying information and evidence; the IBU shall not
be liable with respect to manufacturer information, life
cycle assessment data and evidences.
The EPD was created according to the specifications
of EN 15804+A2. In the following, the standard will be
simplified as EN 15804.
Verification
The standard EN 15804 serves as the core PCR
Independent verification of the declaration and data
according to ISO 14025:2011
Dipl. Ing. Hans Peters internally x externally
(chairman of Institut Bauen und Umwelt e.V.)
Dr. Alexander Röder Vito D'Incognito
(Managing Director Institut Bauen und Umwelt e.V.)) (Independent verifier)
2. Product
2.1 Product description/Product definition For the application and use the respective national
NH/ArmaFlex Smart is the professional, highly-flexible, provisions apply.
closed-cell elastomeric foam insulation (FEF) for 2.2 Application
continuous energy saving and condensation control NH/ArmaFlex Smart is used to insulate pipes, air ducts
purposes. The combination of very low thermal and vessels including fittings and flanges of industrial
conductivity and high resistance to water vapour installations and building equipment.
transmission prevents long-term energy losses and  Condensation control, energy saving and
water vapour ingress and reduces the risk of corrosion noise control in refrigeration and air
under insulation.
conditioning equipment and process plants.
 Energy saving according to local energy-
For the placing on the market of the product in
the European Union/European Free Trade Association saving laws, prevention of heat loss and noise
(EU/EFTA) (with the exception of Switzerland) reduction of heating and plumbing systems.
Regulation (EU) No. 305/2011 (CPR) applies. The  Condensation control and noise reduction in
product needs a declaration of performance taking into service-water and waste-water systems.
consideration EN 14304:2013-04, Thermal insulation
 Condensation control, energy saving and
products for building equipment and industrial
noise control in refrigeration and air-
installations – Factory made flexible elastomeric foam
(FEF) products – Specification and the CE-marking.
2 Environmental Product Declaration Armacell GmbH – NH/ArmaFlex Smart insulation for industrial and building installation
conditioning equipment in the ship-building are not on the candidate list, exceeding 0.1 percentage
sector. by mass: No
Biocide products were added to this construction
product or it has been treated with biocide products
2.3 Technical Data
(this then concerns a treated product as defined by the
(EU) Ordinance on Biocide Products No. 528/2012):
No
Constructional data
Name Value Unit
The products may contain traces of azodicarbonamide
Gross density 62.5 kg/m3
(ADCA). Possible minimal residual amounts are
Water vapour diffusion resistance
≥ 2000 - included in the polymer matrix. A health impairment
factor acc. to EN 12086, EN13469
can be excluded. For the production of insulation
Thermal conductivity 0,040 W/(mK) material based on synthetic rubber, there is presently
(0°C) no alternative to ADCA available.
Maximum service temperature acc. to
+110 °C
EN 14706, EN 14707 Synthetic rubber determines the flexibility;
Minimum service temperature -50 °C Fillers determine the fire properties and firmness;
Tubes: Blowing agent causes the expansion process during
DL-s2, manufacturing;
Reaction to fire acc. to EN 13501-1 d0/ - Accelerator and sulphur enable the vulcanisation;
Sheets: Plasticizers determine the flexibility;
E Flame retardants ensure fire resistance.
Structure-borne sound transmission not
acc. to EN ISO 3822-1 relevant
Weighted sound absorption coefficient not 2.6 Manufacture
αw acc. to EN ISO 11654 relevant ArmaFlex Smart products are manufactured in a
pressureless, continuous and discontinuous production
Insulation materials on the basis of synthetic rubber do process.
not absorb moisture from the air. For this reason the In the first step, a homogenous compound is produced
normal building moisture does not lead to an increase with rubber, additives, ancillary materials, blowing and
in thermal conductivity. vulcanization agents. This is done on the rolling mill or
in the internal mixer followed by the rolling mill.
Performance data of the product in accordance with Rubber extruders are used to process the compounds
the declaration of performance with respect to its to produce raw profiles with defined dimensions. Here
essential characteristics according to EN 14304:2013- exact compliance with the dimensions for the raw
04, Thermal insulation products for building equipment profile is crucial for the dimensional accuracy of the
and industrial installations – Factory made flexible foamed product.
elastomeric foam (FEF) products – Specification In the case of the discontinuous, pressureless
production process, the raw profiles are cut to length
2.4 Delivery status and then foamed in a hot-air oven. In the case of the
Halogen free FEF made of cross-linked elastomer is continuous, pressureless process, the extruded profile
supplied as sheets, tubes and shaped pieces. is fed directly onto a vulcanization line whose energy
Products with self-adhesive backings/closures are source may be hot air.
available; these variations are not included in the In foam production, vulcanization and blowing
calculations. Insulation thicknesses are available for all processes run alongside each other. Both reactions
common pipe diameters up to an outer diameter of 114 are regulated by temperature control. Recipe and
mm (tubes). temperature control determine the properties of the
foam.
2.5 Base materials/Ancillary materials Quality assurance:
EC Certificate of conformity no. 0543 of the
ArmaFlex Smart is a highly flexible insulation material Gütegemeinschaft Hartschaum e.V. Celle.
based on synthetic rubber, which consists of around 20 Quality management system in accordance with EN
basic components. The following table displays the ISO 9001.
composition split into functional substance groups.
Name Value Unit 2.7 Environment and health during
Rubber and polymers 23 % manufacturing
Fillers and pigments 2 % During all manufacturing steps and at all production
Blowing agent 8 % sites of Armacell, the production follows the national
Vulcanisation system, additives, guidelines and regulations. A regenerative thermal
17 %
plasticisers oxidizer is installed to treat exhaust air.
Flame retardant 50 % Certification of the environmental management system
is in accordance with ISO 14001.
This product/article/at least one partial article contains
substances listed in the candidate list (date:
17.01.2022) exceeding 0.1 percentage by mass: No 2.8 Product processing/Installation
The product is installed by using knives. No special
This product/article/at least one partial article contains tools, nor specific protection is necessary.
other CMR substances in categories 1A or 1B which When applying adhesives the information given in the
relevant safety data sheets is to be heeded.
3 Environmental Product Declaration Armacell GmbH – NH/ArmaFlex Smart insulation for industrial and building installation
The recommendations for installing the product According to EN 13501, ArmaFlex Smart is classified
depend on the product and system and are described as a combustible insulation material. Due to its
in the respective documents (e.g. Armaflex application material structure it does not contribute to an
manual) or the data sheets. More details under uncontrollable spread of fire under installation
www.armacell.com. conditions typical on a building site. ArmaFlex Smart
does not drip under practical fire conditions, this
means that fire spread is ruled out. The product is self-
2.9 Packaging extinguishing and therefore only makes a minor
As a rule, ArmaFlex Smart products are packaged in contribution to the actual fire event. There is no
cardboard boxes and transported on reusable pallets possibility of the material self-igniting. ArmaFlex Smart
(For the LCA calculation of this EPD though, 100% does not propagate the fire either horizontally or
incineration is assumed). Over-sized rolls of sheet vertically.
material are packaged in polyethylene (PE) foil. The
cardboard boxes are usually recycled through Fire protection
Interseroh’s dual system. Name Value
Tubes: DL
Euro class / Sheets:
2.10 Condition of use E
When the products are used for the purpose for which Tubes: d0
Burning droplets
they are intended, there are no changes in the material / Sheets: -
composition during use, except in the event of Tubes: s2
Smoke development
extraordinary impacts (see 2.14). / Sheets: -
2.11 Environment and health during use Water
Ingredients: There are no particular aspects of the Armacell insulation materials have a high resistance to
material composition during use. water vapour transmission which keeps possible water
Eurofins Product Testing A/S has tested a wide range vapour transmission processes to a minimum
and varieties of typical FEF (Flexible Elastomeric permanently. Therefore, a significant reduction in the
Foam) products marketed in the EU from CEFEP insulation effect can be ruled out permanently.
(European Group of FEF manufacturers). Sampling, If the insulation material is exposed to water over a
testing and evaluation were performed according to long period of time (e.g. flooding) it should be replaced.
CEN TS 16516, AgBB, ISO 16000-3, ISO 16000-6,
ISO 16000-9, ISO 16000-11 in the latest versions. Mechanical destruction
Based on the loading factor 0.05 m²/m³, which was ArmaFlex Smart insulation materials are flexible foams
determined after consideration of real life applications and thus display limited mechanical stability.
with FEF products (in living rooms) and Therefore, if the material will be subject to greater
recommendation of experts of the test institute, all mechanical impact it should be protected
results were clearly below the limit values. For appropriately, e.g. by a metal jacket or Arma-Chek
example, the determined total volatile organic covering.
compound (TVOC) after 28 days was for all samples ArmaFlex Smart products are not UV resistant. If the
below 100 mg/m3. Certificates are available on material is subject to UV-rays it should be protected
request. accordingly.
2.14 Re-use phase
2.12 Reference service life If removed properly the product can be re-used.
ArmaFlex Smart products are long-lasting products. Correctly sorted material can be ground and used to
Findings show that when used and installed properly manufacture new products (e.g. ArmaSound). For the
they can have an estimated service life of more than LCA calculation of this EPD though, 100% incineration
50 years. It is practically only restricted by the service is assumed.
life of the equipment or whole building, which can
extent that time period. The insulation performance is 2.15 Disposal
almost completely maintained over the entire service Dispose of the materials according to local regulations.
life. The insulation performance is only compromised Regulated by the European Waste Catalogue: Waste
by extraordinary impacts and damage during code 07 02 13 (waste plastic).
construction, Note: Please observe Commission Decision
2001/118/EC.
2.16 Further information
2.13 Extraordinary effects Further information on ArmaFlex® can be found on the
manufacturer’s website www.armacell.com. Detailed
Fire specification clauses for the products are provided at
www.armaflex.de.
3. LCA: Calculation rules
3.1 Declared Unit As additional information and support for installers the
The declaration refers to 1 m³ insulation product. thermal conductivity coefficient (lambda-value) and R-
For the LCA calculations the average density per value per 20 cm thickness per product brand are given.
product brand is used.
Declared unit
4 Environmental Product Declaration Armacell GmbH – NH/ArmaFlex Smart insulation for industrial and building installation
Name Value Unit The reported recipes for the rubber mixes contain
Declared unit 1 m3 specific substances of the rubber industry. For these
Gross density 62.5 kg/m3 materials only partly life cycle inventories are available.
Conversion factor to 1 kg 62.5 - Approximations are used with the consideration of
similar supply chain effort or similar elementary
Thermal conductivity λ : 0.040 W/(mK (0°C) composition. Partly an estimation is modelled using
R-value – thickness: 20 cm: 5.0 (m²K)/W pre-products of the specific material and adding an
energy effort as well as considering the treatment of
production residues for this step in the supply chain.
3.2 System boundary 3.4 Cut-off criteria
The data collection refers to the yearly production in In the assessment, all reported data from the
2020. The following life cycle stages are considered: production process are considered, utilised thermal
energy, and electric power consumption using best
Type of EPD: Cradle-to-Gate with options: available life cycle inventory (LCI) datasets. Thus
material and energy flows contributing less than 1% of
Production A1-A3: mass or energy are considered.
The LCA calculation covers the production of the raw No cut-off criteria are applied in the foreground data in
materials (supply chain – A1), the mixing of raw this study.
materials according to the respective recipes For cut-off criteria in the background system, see the
(MasterBatch) exclusively done in Münster, Germany, information provided in the modelling principles and
the transport (A2) of the MasterBatches to the specific documentations (documentation.gabi-
production facility for foaming and the foaming process software.com).
(A3) in Germany, Spain or Poland, including the
packaging material. 3.5 Background data
Transport A4: The LCA model is created using the GaBi ts Software
Average values for the transport from factory gate to system (v10) for life cycle engineering, developed by
construction site are assumed. Sphera. The GaBi LCI database provides the life cycle
Installation A5: inventory data for several of the raw and process
The installation considers the production of off-cuts, materials obtained from the background system. The
incineration of these off-cuts and the disposal scenario most recent update of the database was 2021 (Service
for the packaging material. Auxiliaries like adhesives or Pack CUP 2021.02)
tapes or energy for installation are not considered.
End-of-life C2, C3: 3.6 Data quality
An incineration scenario for the used and demolished The foreground data collected by the manufacturer are
product, including an assumption for the transport to based on yearly production amounts and
disposal, is covered. extrapolations of measurements on specific machines
Benefits for the next product system D: and plants.
Credits for electrical and thermal energy resulting from Most of the necessary life cycle inventories for the
the waste incineration process of the off-cut material basic materials are available in the GaBi database.
and packaging (A5) and the product (C3) are declared The last update of the database was in 2021 (Service
in module D. Pack CUP 2021.02).
Further LCIs for materials of the supply chain of the
basic materials are approximated with LCIs of similar
materials or estimated by the combination of available
LCIs.
3.3 Estimates and assumptions For electrical and thermal energy regional specific grid
Scenario assumptions: mixes and regional specific supply for natural gas are
Installation (A5): considered.
The additional demand of material for installation
depends on the specific frame conditions of the 3.7 Period under review
building and pipe system to be insulated. Parts of the The production data refer to an average of the year
product can be joined; thus installation off-cut is very 2020.
small. A loss of 1% is assumed.
Transport to customer (A4): 3.8 Allocation
Armacell’s data collectors reported average figures for Allocation of upstream data:
the distribution of their material. Depending on the For all refinery products, allocation by mass and net
country, the transport distance varies from 500 km to calorific value is applied. The specific manufacturing
800 km route of every refinery product is modelled and so the
End-of-life (C2, C3): impacts associated with the production of these
The transport from place of usage to a waste products are calculated individually.
incineration plant is assumed as 100 km. Materials and chemicals used in the manufacturing
After the demolition of the product a current realistic process are modelled using the allocation rule most
End-of-life scenario is the incineration of the material. suitable for the respective product. For further
According to the reported net calorific value of the information on a specific product see
materials and the elementary composition, a partial documentation.gabi-software.com.
stream consideration for the incineration process of Allocation in the foreground data:
PVC-products is applied as an approximation for all Part of the production residues (ca. 2%) are used for
declared products. the manufacturing of a non-declared product
Inventory estimations and approximations: (ArmaSound). These materials leave the process
5 Environmental Product Declaration Armacell GmbH – NH/ArmaFlex Smart insulation for industrial and building installation
without further consideration of any treatment and The credits for thermal and electrical energy are
without credit (cut-off-approach). calculated via inversion of the life cycle inventory of
No further allocation is applied in the software model. European average data.
The overall production of the Armacell production Allocation for waste paper:
facilities comprises further products beside the Paper/corrugated board is used as packaging material
products considered in this study. Data for thermal and and this usually includes a mix of recycled and virgin
electrical energy, as well as auxiliary material, refer to fibres. When modelling the production of paper, the
the declared products only. During data collection the scrap paper that is used in this process has been
allocation is done via mass, area, pieces or time spent assumed to be burden free. Similarly, waste paper
in the machine, depending on the process step and arising in the product life cycle is assumed to be
reasonable split. The data collectors at Armacell recycled. Robust data on paper and cardboard
decided on the distribution basis. recycling are not promptly available and refer to a very
Allocation for waste materials: complex system. Hence, to apply this methodology
Production waste is sent to a waste incineration plant consistently throughout the model, a cut-off approach
and to landfill (Spain). The resulting electrical and has been applied, i.e., input of waste paper is
thermal energy from the incineration process is looped considered without environmental burden, resulting
inside module A1-A3. The quality of the recovered waste paper is not credited. The recycling process and
energy is assumed to be the same as that of the input the production process of paper are merged in the
energy. production process. The C-balance referring to fresh
Landfilling of plastic material is assumed not to deliver fibre is corrected via CO emissions (biotic)
2
any landfill gas. (assumption of final rotting or incineration in the time
All applied incineration processes are displayed via a frame of 100 years).
partial stream consideration for the combustion
process, according to the specific composition of the 3.9 Comparability
incinerated material. For the waste incineration plant Basically, a comparison or an evaluation of EPD data
an R1-value of > 0.6 is assumed. is only possible if all the data sets to be compared
Environmental burden of the incineration of installation were created according to EN 15804 and the building
residues (off-cuts), packaging and the product in the context, respectively the product-specific
end-of-life scenario is assigned to the system (A5 or characteristics of performance, are taken into account.
C3); resulting credits for thermal and electrical energy
are declared in module D. The used background dataset DB has been GaBi
2021 (Service Pack CUP 2021.02).
4. LCA: Scenarios and additional technical information
Characteristic product properties Installation into the building (A5)
Information on biogenic Carbon Name Value Unit
The biogenic carbon content quantifies the amount of Material loss 1 %
biogenic carbon in a construction product leaving the
factory gate, and it shall be separately declared for the
product and any accompanying packaging.If the total
mass of biogenic carbon containing materials is less Estimated service life
than 5 % of the total mass of the product and Name Value Unit
accompanying packaging, the declaration of biogenic Life Span according to the
50 a
carbon content may be omitted. The mass of manufacturer
packaging containing biogenic carbon shall always be
declared.Note: 1 kg biogenic Carbon is equivalent to End of life (C1-C4)
44/12 kg of CO2 Name Value Unit
Energy recovery in WIP 62,5 kg
Information on describing the biogenic Carbon
Content at factory gate Reuse, recovery and/or recycling potentials (D),
Name Value Unit relevant scenario information
Biogenic Carbon Content in product 0 kg C Module D includes the credits of the incineration
Biogenic Carbon Content in processes from A5 (off-cut of product installation,
26.93 kg C
accompanying packaging packaging waste) and C3 (incineration of the product).
The embodied biogenic carbon leaves the system in A waste incineration plant with an R1-value > 0.6 is
Module A5. assumed.
The following technical information serves as a basis
for the declared modules. The values refer to the
declared unit of 1 m³.
Transport to the building site (A4)
Name Value Unit
Litres of fuel 0.2 l/100km
Transport distance 800 km
Capacity utilisation (including empty
85 %
runs)
6 Environmental Product Declaration Armacell GmbH – NH/ArmaFlex Smart insulation for industrial and building installation
5. LCA: Results
The following information on environmental impacts is expressed with the impact category parameters of LCIA
using characterisation factors. The chosen characterisation factors fulfil the requirements of EN 15804.
Disclaimer:
EP-freshwater: This indicator has been calculated as “kg P eq” as required in the characterization model
(EUTREND model, Struijs et al., 2009b, as implemented in ReCiPe;
http://eplca.jrc.ec.europa.eu/LCDN/developerEF.xhtml)
DESCRIPTION OF THE SYSTEM BOUNDARY (X = INCLUDED IN LCA; ND = MODULE OR INDICATOR NOT
DECLARED; MNR = MODULE NOT RELEVANT)
BENEFITS AND
CONSTRUCTI LOADS
PRODUCT STAGE ON PROCESS USE STAGE END OF LIFE STAGE BEYOND THE
STAGE SYSTEM
BOUNDARIES
7 Environmental Product Declaration Armacell GmbH – NH/ArmaFlex Smart insulation for industrial and building installation
lairetam
waR
ylppus tropsnarT
gnirutcafunaM
eht
morf
tropsnarT
etis
eht
ot
etag
ylbmessA esU
ecnanetniaM
riapeR
tnemecalpeR tnemhsibrufeR
ygrene
lanoitarepO esu
retaw
lanoitarepO esu
noitcurtsnoc-eD
noitilomed tropsnarT
gnissecorp
etsaW
lasopsiD -esueR -yrevoceR -gnilcyceR laitnetop
A1 A2 A3 A4 A5 B1 B2 B3 B4 B5 B6 B7 C1 C2 C3 C4 D
X X X X X ND ND MNR MNR MNR ND ND ND X X ND X
RESULTS OF THE LCA - ENVIRONMENTAL IMPACT according to EN 15804+A2: 1 m³ NH/ArmaFlex Smart
insulation for industrial and building installation
Core Indicator Unit A1-A3 A4 A5 C2 C3 D
Global warming potential - total [kg CO2-Eq.] 1.64E+2 4.84E+0 1.07E+2 2.99E-1 1.62E+2 -4.54E+1
Global warming potential - fossil fuels [kg CO2-Eq.] 2.64E+2 4.80E+0 5.16E+0 2.97E-1 1.62E+2 -4.51E+1
Global warming potential - biogenic [kg CO2-Eq.] -1.00E+2 -6.13E-3 1.02E+2 -3.79E-4 3.27E-2 -2.25E-1
GWP from land use and land use change [kg CO2-Eq.] 3.14E-1 3.93E-2 4.13E-3 2.43E-3 3.63E-2 -3.11E-2
Depletion potential of the stratospheric ozone layer [kg CFC11-Eq.] 7.23E-10 6.14E-16 7.31E-12 3.79E-17 2.60E-13 -5.14E-13
Acidification potential, accumulated exceedance [mol H+-Eq.] 4.61E-1 1.40E-2 8.02E-3 8.65E-4 4.39E-2 -5.89E-2
Eutrophication, fraction of nutrients reaching freshwater
end compartment
[kg P4-Eq.] 2.43E-3 1.43E-5 2.54E-5 8.82E-7 4.00E-5 -5.88E-5
Eutrophication, fraction of nutrients reaching marine end
[kg N-Eq.] 1.78E-1 6.37E-3 2.92E-3 3.94E-4 1.47E-2 -1.68E-2
compartment
Eutrophication, accumulated exceedance [mol N-Eq.] 1.74E+0 7.13E-2 3.33E-2 4.41E-3 1.81E-1 -1.79E-1
Formation potential of tropospheric ozone photochemical
[kg NMVOC-Eq.] 6.10E-1 1.26E-2 9.19E-3 7.77E-4 4.26E-2 -4.70E-2
oxidants
Abiotic depletion potential for non-fossil resources [kg Sb-Eq.] 4.59E+3 6.40E+1 5.43E+1 3.95E+0 3.00E+2 -7.83E+2
Abiotic depletion potential for fossil resources [MJ] 1.03E-3 3.66E-7 1.05E-5 2.26E-8 3.70E-6 -7.49E-6
Water (user) deprivation potential, deprivation-weighted [m³ world-Eq
1.06E+1 4.17E-2 2.26E+0 2.58E-3 1.25E+1 -3.45E+0
water consumption (WDP) deprived]
RESULTS OF THE LCA - INDICATORS TO DESCRIBE RESOURCE USE according to EN 15804+A2: 1 m³
NH/ArmaFlex Smart insulation for industrial and building installation
Indicator Unit A1-A3 A4 A5 C2 C3 D
Renewable primary energy as energy carrier [MJ] 1.91E+3 3.57E+0 1.59E+2 2.21E-1 6.70E+1 -1.77E+2
Renewable primary energy resources as material utilization [MJ] 1.37E+2 0.00E+0 -1.37E+2 0.00E+0 0.00E+0 0.00E+0
Total use of renewable primary energy resources [MJ] 2.05E+3 3.57E+0 2.22E+1 2.21E-1 6.70E+1 -1.77E+2
Non-renewable primary energy as energy carrier [MJ] 3.55E+3 6.40E+1 6.35E+1 3.96E+0 1.33E+3 -7.83E+2
Non-renewable primary energy as material utilization [MJ] 1.04E+3 0.00E+0 -9.11E+0 0.00E+0 -1.03E+3 0.00E+0
Total use of non-renewable primary energy resources [MJ] 4.59E+3 6.40E+1 5.44E+1 3.96E+0 3.00E+2 -7.83E+2
Use of secondary material [kg] 4.22E+1 0.00E+0 4.22E-1 0.00E+0 0.00E+0 0.00E+0
Use of renewable secondary fuels [MJ] 0.00E+0 0.00E+0 0.00E+0 0.00E+0 0.00E+0 0.00E+0
Use of non-renewable secondary fuels [MJ] 0.00E+0 0.00E+0 0.00E+0 0.00E+0 0.00E+0 0.00E+0
Use of net fresh water [m³] 1.39E+0 4.09E-3 6.52E-2 2.53E-4 3.27E-1 -1.73E-1
RESULTS OF THE LCA – WASTE CATEGORIES AND OUTPUT FLOWS according to EN 15804+A2:
1 m³ NH/ArmaFlex Smart insulation for industrial and building installation
Indicator Unit A1-A3 A4 A5 C2 C3 D
Hazardous waste disposed [kg] 2.54E-5 3.23E-9 2.58E-7 1.99E-10 5.36E-8 -1.76E-7
Non-hazardous waste disposed [kg] 3.46E+1 9.51E-3 1.53E+0 5.88E-4 9.94E+1 -3.67E-1
Radioactive waste disposed [kg] 8.04E-2 7.75E-5 1.14E-3 4.79E-6 8.82E-3 -5.68E-2
Components for re-use [kg] 0.00E+0 0.00E+0 0.00E+0 0.00E+0 0.00E+0 0.00E+0
Materials for recycling [kg] 0.00E+0 0.00E+0 5.38E+1 0.00E+0 0.00E+0 0.00E+0
Materials for energy recovery [kg] 0.00E+0 0.00E+0 0.00E+0 0.00E+0 0.00E+0 0.00E+0
Exported electrical energy [MJ] 0.00E+0 0.00E+0 2.88E+1 0.00E+0 1.63E+2 0.00E+0
Exported thermal energy [MJ] 0.00E+0 0.00E+0 5.17E+1 0.00E+0 2.98E+2 0.00E+0
RESULTS OF THE LCA – additional impact categories according to EN 15804+A2-optional:
1 m³ NH/ArmaFlex Smart insulation for industrial and building installation
Indicator Unit A1-A3 A4 A5 C2 C3 D
Potential incidence of disease due to PM emissions [Disease
7.75E-6 7.81E-8 1.05E-7 4.82E-9 1.12E-6 -5.07E-7
Incidence]
Potential Human exposure efficiency relative to U235 [kBq U235-
8.49E+0 1.11E-2 1.33E-1 6.85E-4 9.18E-1 -9.32E+0
Eq.]
Potential comparative toxic unit for ecosystems [CTUe] 3.71E+3 4.62E+1 4.24E+1 2.86E+0 2.46E+2 -1.64E+2
Potential comparative toxic unit for humans - cancerogenic [CTUh] 7.09E-8 9.33E-10 9.53E-10 5.76E-11 9.86E-9 -7.46E-9
Potential comparative toxic unit for humans - not cancerogenic [CTUh] 5.27E-6 5.44E-8 6.94E-8 3.36E-9 1.05E-6 -2.94E-7
Potential soil quality index [-] 6.96E+3 2.20E+1 7.24E+1 1.36E+0 6.60E+1 -1.21E+2
Disclaimer 1 – for the indicator “potential Human exposure efficiency relative to U235“.
This impact category deals mainly with the eventual impact of low dose ionizing radiation on human health of the
nuclear fuel cycle. It does not consider effects due to possible nuclear accidents, occupational exposure nor
radioactive waste disposal in underground facilities. Potential ionizing radiation from the soil, from radon and
some construction materials, is also not measured by this indicator.
Disclaimer 2 – for the indicators “abiotic depletion potential for fossil resources”, “abiotic depletion potential for
non-fossil resources”, “water (user) deprivation potential”, “deprivation-weighted water consumption”, “potential
comparative toxic unit for ecosystems”, “potential comparative toxic unit for humans - cancer effects”, “potential
comparative toxic unit for humans – non-cancer effects”, “potential soil quality index
The results of this environmental impact indicator shall be used with care as the uncertainties on these results are
high or as there is limited experience with the indicator.
6. LCA: Interpretation
The supply chain, i.e. the production of the purchased overall green house gas emissions. At the same time a
materials, causes the highest influence on all impact credit (D) of 12% is given to the next system, due to
categories and the primary energy. the use of electrical and thermal energy, gained in the
incineration processes for the product and the off-cut
Global Warming Potential material.
Looking at the GWP for the overall declared life cycle
phases, including production (A1-A3), transport (A4, Further impact categories
C2), installation (losses) (A5) and end-of-life (C3, D), The end-of-life scenarios have less influence on the
the production (A1-A3) contributes to 42%. other considered impact categories than on GWP. The
The production in the supply chain (A1) already main contribution of the considered life cycle phases is
contributes 34% to the total GWP value. Thus, every concentrated on modules A1-A3.
increase in the production yield directly improves the The energy consumption in the foaming step
environmental performance of the products. influences all impact categories; variations depend on
The foaming process (A3), which includes the the national grid mixes for electricity.
electrical and thermal energy for the mixing, the
vulcanisation and blowing step as well as the Primary Energy Demand
production of the packaging materials, shows a The total primary energy demand is for both categories
significant influence on GWP of the life cycle with 8%. (renewable and non-renewable) significantly (> 100%)
Module A5 covers the production and disposal influenced by the production of the modules A1-A3.
(=incineration) of the off-cut material assumed as 1% The other modules play a minor role (C3 with about
loss in respect to the required insulation material. 6%)
Additionally, the emissions of the incineration of
packaging material (plastic, wood) in a waste The share of primary energy bound as material
incineration plant are considered. The installation step accounts for about 19%, which is partly recovered and
contributes with 27% to the overall GWP. credited for in module D (-15%)
As end-of-life scenario, incineration is considered. The
emissions of the product (C3) contribute to 41% of the
7. Requisite evidence
with FEF products (in living rooms) and
7.1 VOC emissions recommendation of the experts of the test institute, all
Eurofins Product Testing A/S has tested a wide range results were clearly below the limit values. For
and varieties of typical FEF (Flexible Elastomeric example the determined total volatile organic
Foam) products marketed in the EU from CEFEP compound (TVOC) after 28 days was for all samples
(European Group of FEF manufacturers). Sampling, below 100 mg/m3. Certificates are available on
testing and evaluation were performed according to request.
CEN TS 16516, AgBB, ISO 16000-3, ISO 16000-6,
ISO 16000-9, ISO 16000-11 in the latest versions. 7.2 Leaching performance
Based on the loading factor 0.05 m²/m³, which were According to EN 13468 is the content of water-soluble
determined after consideration of real life applications
8 Environmental Product Declaration Armacell GmbH – NH/ArmaFlex Smart insulation for industrial and building installation
chloride ions for NH/Armaflex ≤ 80 ppm.
8. References
AgBB EN 14706
Umweltbundesamt Germany, Health-related EN 14706: 2013-01: Thermal insulating products for
Evaluation of Emissions of Volatile Organic building equipment and industrial installations -
Compounds (VVOC, VOC and SVOC) from Building Determination of maximum service temperature
Products
EN 14707
CEFEP EN 14707: 2013-01: Thermal insulating products for
The industry association for FEF and PEF insulation building equipment and industrial installations -
(Celle) in 2012 Determination of maximum service temperature for
preformed pipe insulation
CEN TS 16516
CEN TS 16516:2013-12: Construction products - EN 15801
Assessment of release of dangerous substances - EN 15801: 2010-04: Conservation of cultural property -
Determination of emissions into indoor air Test methods - Determination of water absorption by
capillarity
Comission Decision 2001/118/EC
Amendment to European Waste Catalogue EN 15804
EN 15804:2019+A2, Sustainability of construction
CPR works — Environmental Product Declarations — Core
Regulation (EC) No 305/2011, Construction Products rules for the product category of construction products.
Regulation
EN 29052
EN 826 EN 29052: 1992-08: Acoustics; determination of
EN 826: 2013-05: Thermal insulating products for dynamic stiffness; part 1: materials used under floating
building applications - Determination of compression floors in dwellings
behaviour
EU/EFTA
EN 1606 Regulation (EU) No. 305/2011 (CPR), European
EN 1606: 2013-05: Thermal insulating products for Union/European Free Trade Association (EU/EFTA)
building applications - Determination of compressive
creep Eurofins Product Testing A/S
Eurofins Miljo, Smedeskowej 38, 8464 Galten,
EN 12091 Denmark
EN 12091: 2013-06: Thermal insulating products for
building applications - Determination of freeze-thaw European Waste Catalogue
resistance European Waste Catalogue and Hazardous Waste
List, Commission Decision 2000/532/EC
EN 12086
EN 12086:2013-06: Thermal insulating products for GaBi
building applications - Determination of water vapour GaBi 9 software-system and databases, LBP,
transmission properties University of Stuttgart and Sphera, Leinfelden-
Echterdingen, 2020 (http://documentation.gabi-
EN 13468 software.com/)
EN 13468: 2001-12: Thermal insulating products for
building equipment and industrial installations - IBU 2021
Determination of trace quantities of water soluble General Instructions for the EPD programme of Institut
chloride, fluoride, silicate, and sodium ions and pH Bauen und Umwelt e.V. Version 2.0, Berlin: Institut
Bauen und Umwelt e.V., 2021. www.ibu-epd.com
EN 13469
EN 13469:2013-01: Thermal insulating products for IBU PCR Part A
building equipment and industrial installations - PCR - Part A: Calculation Rules for the Life Cycle
Determination of water vapour transmission properties Assessment and Requirements on the Project Report,
of preformed pipe insulation Institut Bauen und Umwelt e.V., www.ibu-epd.com,
2019.
EN 13501-1
EN 13501-1: 2010-01: Fire classification of IBU PCR PART B
construction products and building elements - Part 1: PCR – Part B: Requirements on the EPD for Insulation
Classification using data from reaction to fire tests materials made of foam plastics, version 1.7, 01-2019 ,
Institut Bauen und Umwelt e.V., www.ibu-epd.com,
EN 14304 2019
EN 14304:2013-04: Thermal insulation products for
building equipment and industrial installations – ISO 3822-1
Factory made flexible elastomeric foam (FEF) products ISO 3822-1: 1999-05: Acoustics - Laboratory tests on
– Specification noise emission from appliances and equipment used in
9 Environmental Product Declaration Armacell GmbH – NH/ArmaFlex Smart insulation for industrial and building installation
water supply installations - Part 1: Method of compounds from building products and furnishing -
measurement Sampling, storage of samples and preparation of test
specimens
ISO 9001
ISO 9001:2014-08: Quality management systems – ISO 16000-3
Requirements ISO 16000-3:2011-10: Determination of formaldehyde
and other carbonyl compounds in indoor air and test
ISO 11654 chamber air - Active sampling method
ISO 11654: 1997-04: Acoustics - Sound absorbers for
use in buildings - Rating of sound absorption ISO 16000-6
ISO 16000-6:2011-12: Indoor air - Part 6:
ISO 14001 Determination of volatile organic compounds in indoor
ISO 14001:2015, Environmental management systems and test chamber air by active sampling on Tenax TA®
— Requirements with guidance for use sorbent, thermal desorption and gas chromatography
using MS or MS-FID
ISO 14025
ISO 14025:2011-10, Environmental labels and ISO 16000-9
declarations — Type III environmental declarations — ISO 16000-9:2006-02: Indoor air - Part 9:
Principles and procedures. Determination of the emission of volatile organic
compounds from building products and furnishing -
ISO 14040 Emission test chamber method
ISO 14040:2009-11: Environmental management –
Life cycle assessment – Principles and framework
REACH
ISO 14044 Regulation (EC) No 1907/2006, Regulation concerning
ISO 14044:2006-10: Environmental management – the Registration, Evaluation, Authorisation and
Life cycle assessment – Requirements and guidelines Restriction of Chemicals (REACH)
ISO 15868
ISO 15686:2011-05, Buildings and constructed assets
- Service life planning
ISO 16000-11
ISO 16000-11: 2006-02: Indoor air - Part 11:
Determination of the emission of volatile organic
10 Environmental Product Declaration Armacell GmbH – NH/ArmaFlex Smart insulation for industrial and building installation
Publisher
Institut Bauen und Umwelt e.V. Tel +49 (0)30 3087748- 0
Panoramastr. 1 Fax +49 (0)30 3087748- 29
10178 Berlin Mail info@ibu-epd.com
Germany Web www.ibu-epd.com
Programme holder
Institut Bauen und Umwelt e.V. Tel +49 (0)30 - 3087748- 0
Panoramastr 1 Fax +49 (0)30 – 3087748 - 29
10178 Berlin Mail info@ibu-epd.com
Germany Web www.ibu-epd.com
Author of the Life Cycle
Assessment Tel +49 711 341817-0
Sphera Solutions GmbH Fax +49 711 341817-25
Hauptstraße 111- 113 Mail info@sphera.com
70771 Leinfelden-Echterdingen Web http://www.sphera.com
Germany
Owner of the Declaration
Armacell GmbH Tel +49-251-7603-0
Robert-Bosch-Str. 10 Fax +49-251-7603-346
48153 Münster Mail info.de@armacell.com
Germany Web www.armacell.de
