ENVIRONMENTAL PRODUCT DECLARATION
as per ISO 14025 and EN 15804+A2
Owner of the Declaration dormakaba International Holding GmbH
Publisher Institut Bauen und Umwelt e.V. (IBU)
Programme holder Institut Bauen und Umwelt e.V. (IBU)
Declaration number EPD-DOR-20220088-CBA8-EN
Issue date 04.05.2022
Valid to 03.05.2027
TS 68/TS 69
dormakaba
www.ibu-epd.com | https://epd-online.com
General Information
dormakaba TS 68/TS 69
Programme holder Owner of the declaration
IBU – Institut Bauen und Umwelt e.V. dormakaba International Holding GmbH
Hegelplatz 1 DORMA Platz 1
10117 Berlin 58256 Ennepetal
Germany Germany
Declaration number Declared product / declared unit
EPD-DOR-20220088-CBA8-EN 1 door closer (1 piece) TS 68/TS 69
This declaration is based on the product category rules: Scope:
Building Hardware products, 01.08.2021 This Environmental Product Declaration refers to a specific door closer
(PCR checked and approved by the SVR) manufactured by dormakaba China Ltd. The production site is located in
Suzhou (China).
Issue date The data represents the year 2020.
The owner of the declaration shall be liable for the underlying information
04.05.2022
and evidence; the IBU shall not be liable with respect to manufacturer
information, life cycle assessment data and evidences.
Valid to
The EPD was created according to the specifications of EN 15804+A2. In
03.05.2027 the following, the standard will be simplified as EN 15804.
Verification
The standard EN 15804 serves as the core PCR
Independent verification of the declaration and data according to ISO
14025:2011
internally X externally
Dipl.-Ing. Hans Peters
(Chairman of Institut Bauen und Umwelt e.V.)
Florian Pronold Dr.-Ing. Wolfram Trinius,
(Managing Director Institut Bauen und Umwelt e.V.) (Independent verifier)
1 Environmental Product Declaration - dormakaba - TS 68/TS 69
Product
Product description/Product definition
The TS 68 and TS 69 are low-cost door closers which can be
universally used on all common door types. The door closers
are particularly quick and easy to install. For the use and
application of the product the respective national provisions at
the place of use apply. The standards which can be applied are
the following:
• EN 1154
• EN 1634-1
Application
The door closers are used for any standard door and almost all
mounting position.
Technical Data
The door closers have following technical properties:
Performance data of the product with respect to its
characteristics in accordance with the relevant technical
provision which can be applied are mentioned above.
Base materials/Ancillary materials
The major material compositions including the packaging of the
product are listed below:
Name Value Unit
Steel 66 %
Aluminium 19 %
Paper 7 %
Plastics 5 %
Lubricants 3 %
The product includes partial articles which contain substances
listed in the Candidate List of REACH Regulation
1907/2006/EC (date: 17.01.2022) exceeding 0.1 percentage by
mass: yes
• Lead (Pb): 7439-92-1 (CAS-No.) is included in some of
the alloys used. The concentration of lead in each
individual alloy does not exceed 4.0% (by mass).
The Candidate List can be found on the ECHA website
address: https:echa.europa.eu/de/home.
Reference service life
The reference service life of the TS 68/TS 69 door closers
depend on the traffic pattern and degree of usage of the door.
These closers are rated to EN 1154, meaning they are
designed to withstand a minimum of 500,000 cycles. The
reference service life amounts for 20 years. This corresponds
with approx. 25,000 cycles per year.
2 Environmental Product Declaration - dormakaba - TS 68/TS 69
LCA: Calculation rules
final residues during the construction process stage.
Declared Unit
The declared unit is 1 piece of the product: TS68/TS 69. End-of-life stage– Modules C1-C4 and D
Name Value Unit The end-of-life stage includes:
Declared unit 1 piece/product — C1, de-construction, demolition:
— C2, transport to waste processing;
Mass of declared Product 2.07 kg
— C3, waste processing for reuse, recovery and/or
recycling;
System boundary
— C4, disposal;
The type of EPD is: cradle to gate with options,
including provision and all transport, provision of all
modules C1–C4, and module D
materials, products and related energy and water use.
(A1–A3 + C + D and additional modules: A4 + A5)
Module D (Benefits and loads beyond the system
boundary) includes:
Production - Module A1-A3
— D, recycling potentials, expressed as net impacts
The product stage includes:
and benefits.
— A1, raw material extraction, processing and
mechanical treatments, processing of secondary Geographic Representativeness
material input (e.g. recycling processes), Land or region, in which the declared product system is
— A2, transport to the manufacturer, manufactured, used or handled at the end of the product´s
— A3, manufacturing and assembly lifespan: China
including provision of all materials, products and energy, as well
as waste processing up to the end-of waste state.
Comparability
Construction stage - Modules A4-A5 Basically, a comparison or an evaluation of EPD data is only
The construction process stage includes: possible if all the data sets to be compared were created
— A4, transport to the building site; according to EN 15804 and the building context, respectively
— A5, installation into the building; the product-specific characteristics of performance, are taken
including provision of all materials, products and energy, as well into account.
as waste processing up to the end-of waste state or disposal of
LCA: Scenarios and additional technical information
Reference service life
Characteristic product properties of biogenic carbon
Name Value Unit
Information on describing the biogenic Carbon Content at
Life Span according to the manufacturer 20 a
factory gate
Name ValueUnit End of life (C1-C4)
Biogenic carbon content in accompanying kg C1: The product dismantling from the building is done manually
0.05
packaging C without environmental burden.
C2: Transport to waste treatment at end of life is 50km.
Additional technical information for the declared modules. Name Value Unit
Transport to the building site (A4) Collected separately waste type 1.93 kg
Recycling 1.75 kg
Name Value Unit
Energy recovery 0.1 kg
Litres of fuel truck (per piece) 0.00276l/100km
Final deposition 0,08 kg
Transport distance (truck) 1500 km
Capacity utilisation (including empty runs) 55 % Reuse, recovery and/or recycling potentials (D), relevant
average scenario information
Transport distance (ship) 10000 km
Name Value Unit
Installation into the building (A5) Recycling 100 %
Name ValueUnit Collection rate is 100%.
Output substances following waste treatment on
0.136 kg
site (paper packaging)
3 Environmental Product Declaration - dormakaba - TS 68/TS 69
LCA: Results
DESCRIPTION OF THE SYSTEM BOUNDARY (X = INCLUDED IN LCA; MND = MODULE OR INDICATOR NOT DECLARED; MNR
= MODULE NOT RELEVANT)
Benefits and
Construction loads beyond
Product stage Use stage End of life stage
process stage the system
boundaries
la ire ta m w a Ry lp p u s tro p s n a rT g n iru tc a fu n a M e h t m o rf tro p s n a rTe tis e h t o t e ta g y lb m e s s A e s U e c n a n e tn ia M ria p e R tn e m e c a lp e R tn e m h s ib ru fe R y g re n e la n o ita re p Oe s u re ta w la n o ita re p Oe s u n o itc u rts n o c -e Dn o itilo m e d tro p s n a rT g n is s e c o rp e ts a W la s o p s iD -e s u e R-y re v o c e R-g n ilc y c e Rla itn e to p
A1 A2 A3 A4 A5 B1 B2 B3 B4 B5 B6 B7 C1 C2 C3 C4 D
X X X X X MND MND MNR MNR MNR MND MND X X X X X
RESULTS OF THE LCA - ENVIRONMENTAL IMPACT according to EN 15804+A2: 1 door closer
Parameter Unit A1-A3 A4 A5 C1 C2 C3 C4 D
GWP-total kg CO 2 eq 1.46E+01 3.39E-01 1.93E-01 0 8E-03 2.46E-01 1E-03 -2.76E+00
GWP-fossil kg CO 2 eq 1.48E+01 3.27E-01 5E-03 0 8E-03 2.46E-01 1E-03 -2.75E+00
GWP-biogenic kg CO 2 eq -2.09E-01 1.2E-02 1.88E-01 0 3.72E-04 5.73E-06 4.33E-06 -8E-03
GWP-luluc kg CO 2 eq 8.02E-03 7.57E-06 3.17E-06 0 1.91E-07 1.39E-05 3.65E-06 -4.64E-04
ODP kg CFC11 eq 2.74E-10 3.38E-17 3.48E-17 0 8.49E-19 1.24E-16 4.7E-18 -1.93E-11
AP mol H+ eq 6.8E-02 3E-03 5.4E-05 0 8.04E-06 4.38E-05 9.09E-06 -1E-02
EP-freshwater kg P eq 1.14E-05 7.08E-08 6.8E-09 0 1.72E-09 1.98E-08 2.18E-09 -1.55E-06
EP-marine kg N eq 1.1E-02 7.41E-04 1.95E-05 0 2.56E-06 9.87E-06 2.34E-06 -1E-03
EP-terrestrial mol N eq 1.24E-01 8E-03 2.43E-04 0 2.85E-05 1.99E-04 2.57E-05 -1.4E-02
kg NMVOC
POCP 3.5E-02 2E-03 5.17E-05 0 7.24E-06 2.73E-05 7.08E-06 -4E-03
eq
ADPE kg Sb eq 1.34E-04 9.52E-09 5.49E-10 0 2.41E-10 1.7E-09 1.14E-10 -1.4E-05
ADPF MJ 1.58E+02 4.5E+00 6.1E-02 0 1.14E-01 1.14E-01 1.7E-02 -3.87E+01
m3 world eq
WDP 2.64E+00 6.3E-04 2.4E-02 0 1.58E-05 2.5E-02 1.33E-04 -1.38E-01
deprived
GWP = Global warming potential; ODP = Depletion potential of the stratospheric ozone layer; AP = Acidification potential of land and water; EP =
Eutrophication potential; POCP = Formation potential of tropospheric ozone photochemical oxidants; ADPE = Abiotic depletion potential for non-fossil
resources; ADPF = Abiotic depletion potential for fossil resources; WDP = Water (user) deprivation potential)
RESULTS OF THE LCA - INDICATORS TO DESCRIBE RESOURCE USE according to EN 15804+A2: 1 door closer
Parameter Unit A1-A3 A4 A5 C1 C2 C3 C4 D
PERE MJ 2.04E+01 1.4E-02 1.64E+00 0 3.59E-04 1.92E-01 2E-03 -1.68E+01
PERM MJ 1.79E+00 0 -1.63E+00 0 0 -1.62E-01 0 0
PERT MJ 2.22E+01 1.4E-02 1.1E-02 0 3.59E-04 3E-02 2E-03 -1.68E+01
PENRE MJ 1.54E+02 4.5E+00 6.1E-02 0 1.14E-01 3.84E+00 1.7E-02 -3.87E+01
PENRM MJ 3.73E+00 0 0 0 0 -3.73E+00 0 0
PENRT MJ 1.58E+02 4.5E+00 6.1E-02 0 1.14E-01 1.14E-01 1.7E-02 -3.87E+01
SM kg 1.32E+00 0 0 0 0 0 0 0
RSF MJ 0 0 0 0 0 0 0 0
NRSF MJ 0 0 0 0 0 0 0 0
FW m3 6.81E-02 2.57E-05 5.63E-04 0 6.45E-07 6.01E-04 4.19E-06 -3E-02
PERE = Use of renewable primary energy excluding renewable primary energy resources used as raw materials; PERM = Use of renewable primary
energy resources used as raw materials; PERT = Total use of renewable primary energy resources; PENRE = Use of non-renewable primary energy
excluding non-renewable primary energy resources used as raw materials; PENRM = Use of non-renewable primary energy resources used as raw
materials; PENRT = Total use of non-renewable primary energy resources; SM = Use of secondary material; RSF = Use of renewable secondary fuels;
NRSF = Use of non-renewable secondary fuels; FW = Use of net fresh water
RESULTS OF THE LCA – WASTE CATEGORIES AND OUTPUT FLOWS according to EN 15804+A2:
1 door closer
Parameter Unit A1-A3 A4 A5 C1 C2 C3 C4 D
HWD kg 1.01E-05 4.38E-10 8.97E-11 0 1.11E-11 4.34E-10 2.53E-10 -2.85E-07
NHWD kg 1.59E+00 4.61E-04 6E-03 0 1.17E-05 2.6E-02 8.4E-02 -6.2E-01
RWD kg 1.83E-03 4.87E-06 3.2E-06 0 1.23E-07 4.23E-06 1.89E-07 -4E-03
CRU kg 0 0 0 0 0 0 0 0
MFR kg 0 0 0 0 0 1.74E+00 0 0
MER kg 0 0 0 0 0 0 0 0
EEE MJ 0 0 2.92E-01 0 0 0 0 0
EET MJ 0 0 5.29E-01 0 0 0 0 0
HWD = Hazardous waste disposed; NHWD = Non-hazardous waste disposed; RWD = Radioactive waste disposed; CRU = Components for re-use;
MFR = Materials for recycling; MER = Materials for energy recovery; EEE = Exported electrical energy; EET = Exported thermal energy
4 Environmental Product Declaration - dormakaba - TS 68/TS 69
RESULTS OF THE LCA – additional impact categories according to EN 15804+A2-optional:
1 door closer
Parameter Unit A1-A3 A4 A5 C1 C2 C3 C4 D
Disease
PM 1.67E-06 4.4E-08 2.99E-10 0 4.23E-11 5.58E-10 1.13E-10 -1.56E-07
incidence
IR kBq U235 eq 2.35E-01 6.97E-04 4.95E-04 0 1.75E-05 3.81E-04 1.95E-05 -8.15E-01
ETP-fw CTUe 5.92E+01 3.19E+00 2.9E-02 0 8.1E-02 4.3E-02 9E-03 -1.35E+01
HTP-c CTUh 5.21E-09 6E-11 1.53E-12 0 1.52E-12 3.7E-12 1.41E-12 -4.88E-10
HTP-nc CTUh 1.64E-07 2.62E-09 6.62E-11 0 6.5E-11 3.75E-10 1.55E-10 -9.62E-09
SQP SQP 3.99E+01 1.2E-02 1.6E-02 0 2.93E-04 3.4E-02 3E-03 -1.32E+00
PM = Potential incidence of disease due to PM emissions; IR = Potential Human exposure efficiency relative to U235; ETP-fw = Potential comparative
Toxic Unit for ecosystems; HTP-c = Potential comparative Toxic Unit for humans (cancerogenic); HTP-nc = Potential comparative Toxic Unit for humans
(not cancerogenic); SQP = Potential soil quality index
Disclaimer 1 – for the indicator “Potential Human exposure efficiency relative to U235”. This impact category deals mainly with the
eventual impact of low-dose ionizing radiation on human health of the nuclear fuel cycle. It does not consider effects due to possible
nuclear accidents, occupational exposure or radioactive waste disposal in underground facilities. Potential ionizing radiation from the
soil, radon and from some construction materials is also not measured by this indicator.
Disclaimer 2 – for the indicators “abiotic depletion potential for non-fossil resources”, “abiotic depletion potential for fossil resources”,
“water (user) deprivation potential, deprivation-weighted water consumption”, “potential comparative toxic unit for ecosystems”,
“potential comparative toxic unit for humans – cancerogenic”, “Potential comparative toxic unit for humans - not cancerogenic”,
“potential soil quality index”. The results of this environmental impact indicator shall be used with care as the uncertainties on these
results are high as there is limited experience with the indicator.
References
Standards of the Council on the Registration,
Evaluation, Authorisation and Restriction of Chemicals
EN 15804 (REACH).
EN 15804:2012+A1 2013, Sustainability of construction works
— Environmental Product Declarations — Core rules for the Further References
product category of construction products.
GaBi
ISO 14025 Sphera Solutions GmbH
EN ISO 14025:2011, Environmental labels and declarations — Gabi Software System and Database for Life Cycle
Type III environmental declarations — Principles and Engineering 1992-2020
procedures. Version 10.0.0.71
University of Stuttgart
IBU 2021 Leinfelden-Echterdingen
Institut Bauen und Umwelt e.V.: General Instructions for the
EPD programme of Institut Bauen und Umwelt e.V., Version GaBi ts documentation
2.0, Berlin: Institut Bauen und Umwelt e.V., 2021 www.ibu- GaBi life cycle inventory data documentation
epd.com (https://www.gabi-software.com/support/gabi/gabidatabase-
2020-lci-documentation/).
EN 1154
EN 1154-2003; Building hardware - Controlled door closing LCA-tool dormakaba
devices - Requirements and test methods. LCA-tool, IBU-DOR-202104-LT1-EN,
Developed by Sphera Solutions GmbH.
EN 1634-1
EN 1634-1:2018; Fire resistance and smoke control tests for PCR Part A
door and shutter assemblies, openable windows and elements PCR – Part A: Calculation Rules for the Life Cycle Assessment
of building hardware - Part 1: Fire resistance test for door and and Requirements on the Project Re-port according to EN
shutter assemblies and openable windows. 15804+A2:2019, Version 1.0, 2020, Institut Bauen und Umwelt
e.V., www.ibu-epd.com.
EN 15804+A2
EN 15804:2019+A2 (in press), Sustainability of construction PCR Part B
works — Environmental Product Declarations — Core rules for PCR – Part B: Requirements on the EPD for Building
the product category of construction products. Hardware product, 2021, Institut Bauen und
Umwelt e.V., www.ibu-epd.com.
REACH Regulation 1907/2006/EC
Regulation (EC) No 1907/2006 of the European Parliament and
5 Environmental Product Declaration - dormakaba - TS 68/TS 69
Publisher
Institut Bauen und Umwelt e.V. +49 (0)30 3087748- 0
Hegelplatz 1 info@ibu-epd.com
10117 Berlin www.ibu-epd.com
Germany
Programme holder
Institut Bauen und Umwelt e.V. +49 (0)30 3087748- 0
Hegelplatz 1 info@ibu-epd.com
10117 Berlin www.ibu-epd.com
Germany
Author of the Life Cycle Assessment
Sphera Solutions GmbH +49 711 341817-0
Hauptstraße 111- 113 info@sphera.com
70771 Leinfelden-Echterdingen www.sphera.com
Germany
Owner of the Declaration
dormakaba International Holding GmbH +49 2333 793-0
DORMA Platz 1 info.de@dormakaba.com
58256 Ennepetal www.dormakaba.com
Germany
6 Environmental Product Declaration - dormakaba - TS 68/TS 69
