ENVIRONMENTAL PRODUCT DECLARATION
as per ISO 14025 and EN 15804+A1
Owner of the Declaration Isolparma
Programme holder Institut Bauen und Umwelt e.V. (IBU)
Publisher Institut Bauen und Umwelt e.V. (IBU)
Declaration number EPD-ISL-20200305-CBA2-EN
Issue date 18.12.2020
Valid to 17.12.2025
ISOLPARMA RFM average thick panel
Isolparma
www.ibu-epd.com | https://epd-online.com
Umwelt Produktdeklaration Name des Herstellers – Name des Produkts
General Information
Isolparma ISOLPARMA RFM insulation panel
Programme holder Owner of the declaration
IBU – Institut Bauen und Umwelt e.V. Isolparma
Panoramastr. 1 Piazza L. Da Porto, n. 14
10178 Berlin
Germany 35131 | Padova | PD | Italy
Declaration number Declared product / declared unit
EPD-ISL-20200305-CBA2-EN ISOLAPARMA RFM expanded rigid polyurethane
foam, covered on both sides by multilayer facer based
on aluminium, facers, and produced by Isolparma. The
EPD applies to 1 m2 of average 61 mm thickness PUR
sandwich board, i.e. 0.061 m3, with an average density
between foam and facing of 34.7 kg/m3.
This declaration is based on the product Scope:
category rules: Isolaparma produces ISOLPARMA RFM that is a high
Insulating materials made of foam plastics, 06.2017 performance insulation board manufactured from
(PCR checked and approved by the SVR) closed cell expanded rigid polyurethane foam, covered
on both sides by multilayer facers based on
aluminium.The data have been provided by the only
Issue date
Isolparma factory that is located in Padova (Italy) for
18.12.2020
the year 2019.
Valid to
The owner of the declaration shall be liable for the
17.12.2025
underlying information and evidence; the IBU shall not
be liable with respect to manufacturer information, life
cycle assessment data and evidences.
The EPD was created according to the specifications
of EN 15804+A1. In the following, the standard will be
simplified as EN 15804.
Verification
The standard EN 15804 serves as the core PCR
Independent verification of the declaration and data
according to ISO 14025:2010
Dipl. Ing. Hans Peters internally x externally
(chairman of Institut Bauen und Umwelt e.V.)
Dr. Alexander Röder Prof. Dr. Birgit Grahl
(Managing Director Institut Bauen und Umwelt e.V.)) (Independent verifier)
Product
Product description/Product definition panel, made of an insulation component in
Isolparma’s thermo insulation panels are mainly used polyurethane foam using blowing agent Pentane-
in the building/construction sector and that of industrial based, covered on both sides with multilayer facers
insulation. based on aluminium.
The panels are made of thermo-setting closed cells The gas-tight properties of the facing allow the highest
polyurethane foam (PU) supplied with various types of thermal insulation to be achieved and maintained over
flexible facers on both sides of the panel. The time.
nature/type of facer contributes to the performance The panel is produced in standard dimensions of 600 x
characteristics of the product and its application. 1200 mm and straight finished edges. Upon request
Expanded rigid polyurethane foam is distinguished by and for minimum quantities, the panels may be
its’ excellent thermo insulation performance, produced in various dimensions, and the borders may
mechanical resistance, workability, lightness, and be rabbeted along the sides. The surface of the panel
durability. may be evened off by sandpaper in order to allow
The performance of Isolparma’s panels is determined installation to uneven surfaces. Isolparma RFM panel
based on the European norm EN is produced by a certified company with systems: ISO
13165:2012+A2:2016 Thermal insulation products for 9001, ISO 45001, ISO 14001 in its entire line of
buildings - Factory made rigid polyurethane foam (PU) products.
products - Specification.
This EPD refers to Isolparma’s RFM average thick
2 Environmental Product Declaration Isolparma srl – Isolparma RFM
For the placing on the market of the product in the The PU board for insulation:
European Union/European Free Trade Association  This product/article/at least one partial article
(EU/EFTA) (with the exception of Switzerland) contains substances listed in the candidate
Regulation (EU) No. 305/2011 (CPR) applies. The
list (date: 17.11.2020) exceeding 0.1
product needs a Declaration of Performance (DoP)
percentage by mass: no
taking into consideration EN 13165:2012+A2:2016
Thermal insulation products for building- factory made  This product/article/at least one partial article
rigid polyurethane foam (PU) products - doesn’t contain other CMR substances in
Specification and the CE-marking. For the application categories 1A or 1B which are not on the
and use the respective national provisions apply. candidate list, exceeding 0.1 percentage by
Application
mass: no
The ISOLPARMA RFM panel is recommended for
 Biocide products were added to this
insulaing: wall, floor and roof insulation under
construction product or it has been treated
waterproof membrane with cold applied.
ISOLPARMA RFM is used to make Isolparma Isoplan with biocide products (this then concerns a
M1, M3 and M4 products. treated product as defined by the (EU)
Ordinance on Biocide Products No.
Technical Data 528/2012): no
The data provided by the Declaration of Performance
apply. In this Life Cycle Assessment, a PU insulation
board with the following properties has been regarded: Additional declaration according to quoted law: The
product is compliant with all requirements indicated at
Constructional data chapter 2.4.2.9 of the PANGPP 2017:
Name Value Unit  Any blowing agent with Ozone depletion
Gross density 34.7 kg/m3 potential >0 is not used in production
Declared Thermal conductivity λD acc.  Catalysts lead-based are not used in
0.022 W/mK
to /EN 13165/
production
Compressive strength at 10%
> 150 kPa  Flame retardants used in production
deformation acc. to /EN 826/
(belonging to the Organophosphorus class)
Tensile strength perpendicular to the
face acc. to /EN 1607/ > 35 kPa are not banned by any national or European
Water absorption by total immersion regulation
< 1 Vol.-%
acc. to /EN 12087/  According to the raw materials declarations of
Water absorption by partial immersion suppliers the minimum amount of recycled
< 0.1 kg/m²
acc. to /EN 1609/ raw materials based on the insulation board
Water vapour diffusion resistance
146 (PU foam and facers) weight is 3 %w and the
factor μ acc. to /EN 12086/
minimum amount of recycled raw materials
Euroclass reaction to fire acc. to /EN
F based on the PU insulation foam weight is 4
11925/
%w (note: this information is not explicitly
This provides a thermal resistance R = 2.65 m² k/W. considered in the LCA and not included in the
EPD tables that only refer to recycling content
in the foreground system).
Base materials/Ancillary materials
Core material (about 83.7 % of the weight of the
Reference service life
declared unit):
The durability of insulation panels is normally at least
Closed-cell Polyiso (PIR) rigid foam made from MDI
as long as the lifetime of the building in which it is
(50-65 %), polyols (20-30 %), pentane (4-5 %) and
used. The experimental data show that the reference
additives (4-7 %).
life is longer than 50 years, Clima 2019.
Facing (about 16.3 % of the weight of the declared
unit): multilayer facer consisting of PE and PP (20-40
%), aluminium (10-15%) and paper (55-75%).
LCA: Calculation rules
Declared Unit Declared thermal conductivity λD 0.023 W/mK
The declared unit is 1 m² with an average thickness of Layer thickness 0.061 m
61 mm, e. g. 0.061 m³. Conversion factor to 1 kg 2.12 kg/m²
Corresponding conversion factors are listed in the Weight of declared unit 2.12 kg/m²
table below. The LCI data used in this report refer to an average
product having an average thickness (materials in the
Declared unit recipes of different thicknesses are weighted according
Name Value Unit to the relative production in square meters). The type
Declared unit 1 m2 of declaration is 1 c - declaration of an average product
Gross density 34.7 kg/m3 from a manufacturer's plant.
Volume 0.061 m³
Grammage 2.12 kg/m2
3 Environmental Product Declaration Isolparma srl – Isolparma RFM
System boundary Comparability
This life cycle assessment for the production of the Basically, a comparison or an evaluation of EPD data
polyurethane insulation board considers the life cycle is only possible if all the data sets to be compared
from the supply of raw materials to the manufacturer´s were created according to EN 15804 and the building
gate (cradle-to-gate with options). It also includes the context, respectively the product-specific
transport to the construction site, the installation and characteristics of performance, are taken into account.
the end-of-life stage of the used PU thermal insulation
board. The life cycle is split into the following individual For life cycle modelling of the considered products,
phases: the /GaBi 9 2020 has been used.
A1 - Raw material formulation
A2 - Raw material transport
A3 - Production of the insulation board and packaging
material
A4 - Transport to the construction site
A5 - Emissions and cutting losses during installation
and packaging disposal
C2 - Transport to end of life
C3/C4 - End-of-Life: waste management (thermal
recovery, landfill)
D - Benefits and loads beyond system boundary
LCA: Scenarios and additional technical information
Other resources - kg
Electricity consumption - kWh
Transport to the building site (A4) Other energy carriers - MJ
The distances calculated are weighted average Material loss - kg
distances according to the overall sales distribution;
such distribution is considered similar for all Isolparma Replacement (B4) / Refurbishment (B5)
products. Name Value Unit
Name Value Unit Number/
Truck with a capacity of 17.3 tons 271 km Replacement cycle - RSL
Ferry with a capacity of 1200-10000 144 km Electricity consumption - kWh
dwt payload capacity Litres of fuel - l/100km
Ship with a capacity of 27500 dwt
11000 km Replacement of worn parts - kg
payload capacity tons
Plane with a capacity of 22 ton 0 km
Reference service life
Installation into the building (A5) Name Value Unit
Name Value Unit Reference service life - a
Material loss 0.0423 kg
Life Span (according to BBSR) - a
VOC in the air Pentane 1.27E-06 kg Life Span according to the
- a
manufacturer
Declared product properties (at the
Use or application of the installed product (B1) see - -
gate) and finishes
section 2.12 "Use"
Design application parameters (if
Name Value Unit
instructed by the manufacturer),
including the references to the - -
Maintenance (B2)
appropriate practices and application
Name Value Unit
codes
Information on maintenance - -
An assumed quality of work, when
Number/
Maintenance cycle - installed in accordance with the - -
RSL
manufacturer’s instructions
Water consumption - m3
Outdoor environment, (for outdoor
Auxiliary - kg
applications), e.g. weathering,
Other resources - kg
pollutants, UV and wind exposure, - -
Electricity consumption - kWh building orientation, shading,
Other energy carriers - MJ temperature
Material loss - kg Indoor environment (for indoor
applications), e.g. temperature, - -
Repair (B3) moisture, chemical exposure
Name Value Unit Usage conditions, e.g. frequency of
Information on the repair process - - use, mechanical exposure - -
Information on the inspection process - - Maintenance e.g. required frequency,
Number/ type and quality and replacement of - -
Repair cycle -
RSL components
Water consumption - m3
Auxiliary - kg
4 Environmental Product Declaration Isolparma srl – Isolparma RFM
Operational energy use (B6) and Operational water
use (B7)
Name Value Unit
Water consumption - m3
Electricity consumption - kWh
Other energy carriers - MJ
Equipment output - kW
End of life (C1-C4)
The results for the end-of-life are declared for the 2
different scenarios:
Name Value Unit
Scenario No 1: Material Incineration 100 %
Scenario No 2: Landfill 100 %
C4: Disposal scenarios used is divided into the 2
sub-scenarios:
1) Incineration 100% (C4/1)
2) Landfilling 100% (C4/2)
D: Benefits and loads beyond system boundary is
divided into the 2 sub-scenarios:
1) Incineration 100% (D1)
2) Landfilling 100% (D2)
Reuse, recovery and/or recycling potentials (D),
relevant scenario information
Name Value Unit
Module D includes credits from recycling materials of
insulation panels and packaging, energy credits from
thermal recovery of the packaging. The results are
declared for the same 3 different scenarios described
above.
5 Environmental Product Declaration Isolparma srl – Isolparma RFM
LCA: Results
The tables below show the results of the LCA. Basic information on all declared modules provides chapter 4.
There are two scenarios for the end-of-life (C3, C4 and D) analyzed: Scenario 1 considers 100% incineration,
Scenario 2 considers 100% landfill disposal.
For SM, RSF, NRSF,CRU indicators only the foreground system is considered.
DESCRIPTION OF THE SYSTEM BOUNDARY (X = INCLUDED IN LCA; MND = MODULE NOT DECLARED;
MNR = MODULE NOT RELEVANT)
BENEFITS AND
CONSTRUCTI LOADS
PRODUCT STAGE ON PROCESS USE STAGE END OF LIFE STAGE BEYOND THE
STAGE SYSTEM
BOUNDARIES
6 Environmental Product Declaration Isolparma srl – Isolparma RFM
lairetam
waR
ylppus tropsnarT
gnirutcafunaM
eht
morf
tropsnarT
etis
eht
ot
etag
ylbmessA esU
ecnanetniaM
riapeR
tnemecalpeR tnemhsibrufeR
ygrene
lanoitarepO esu
retaw
lanoitarepO esu
noitcurtsnoc-eD
noitilomed tropsnarT
gnissecorp
etsaW
lasopsiD -esueR -yrevoceR -gnilcyceR laitnetop
A1 A2 A3 A4 A5 B1 B2 B3 B4 B5 B6 B7 C1 C2 C3 C4 D
X X X X X MND MND MNR MNR MNR MND MND MND X X X X
RESULTS OF THE LCA - ENVIRONMENTAL IMPACT according to EN 15804+A1: 1 m² RFM average thick
panel
Parameter Unit A1-A3 A4 A5 C2 C3/1 C3/2 C4/1 C4/2 D/1 D/2
GWP [kg CO2-Eq.] 5.47E+0 1.73E-1 9.77E-3 9.77E-3 0.00E+0 0.00E+0 4.31E+0 2.23E-1 -2.39E+0 -6.35E-2
ODP [kg CFC11-Eq.] 9.54E-6 1.91E-7 7.06E-14 7.06E-14 0.00E+0 0.00E+0 5.33E-11 3.96E-11 -1.31E-9 -1.42E-11
AP [kg SO2-Eq.] 1.44E-2 3.38E-4 2.44E-5 2.44E-5 0.00E+0 0.00E+0 1.79E-3 3.78E-4 -5.46E-3 -1.08E-4
EP [kg (PO4)3--Eq.] 1.95E-3 4.81E-5 5.66E-6 5.66E-6 0.00E+0 0.00E+0 4.24E-4 9.45E-5 -5.08E-4 -1.16E-5
POCP [kg ethene-Eq.] 3.59E-3 7.59E-5 -6.73E-6 -6.73E-6 0.00E+0 0.00E+0 1.22E-4 6.22E-5 -4.38E-4 -1.35E-5
ADPE [kg Sb-Eq.] 1.32E-5 2.73E-7 7.30E-10 7.30E-10 0.00E+0 0.00E+0 5.76E-8 3.16E-8 -6.25E-7 -1.74E-8
ADPF [MJ] 1.32E+2 2.79E+0 1.34E-1 1.34E-1 0.00E+0 0.00E+0 1.66E+0 1.16E+0 -2.94E+1 -1.39E+0
GWP = Global warming potential; ODP = Depletion potential of the stratospheric ozone layer; AP = Acidification potential of land and water; EP =
Caption Eutrophication potential; POCP = Formation potential of tropospheric ozone photochemical oxidants; ADPE = Abiotic depletion potential for non-
fossil resources; ADPF = Abiotic depletion potential for fossil resources
RESULTS OF THE LCA - INDICATORS TO DESCRIBE RESOURCE USE according to EN 15804+A1: 1 m²
RFM average thick panel
Parameter Unit A1-A3 A4 A5 C2 C3/1 C3/2 C4/1 C4/2 D/1 D/2
PERE [MJ] 2.01E+1 IND 4.34E-1 IND IND IND 3.93E-1 IND IND IND
PERM [MJ] 1.82E-2 IND -1.10E-2 IND IND IND 0.00E+0 IND IND IND
PERT [MJ] 2.01E+1 2.71E-2 4.23E-1 7.75E-3 0.00E+0 0.00E+0 3.93E-1 3.25E-1 -9.07E+0 -1.69E-1
PENRE [MJ] 6.77E+1 IND 2.16E+0 IND IND IND 7.21E+1 IND IND IND
PENRM [MJ] 7.19E+1 IND -1.97E+0 IND IND IND -6.99E+1 IND IND IND
PENRT [MJ] 1.40E+2 6.00E-1 1.86E-1 1.35E-1 0.00E+0 0.00E+0 2.17E+0 1.54E+0 -4.16E+1 -1.55E+0
SM [kg] 0.00E+0 0.00E+0 0.00E+0 0.00E+0 0.00E+0 0.00E+0 0.00E+0 0.00E+0 0.00E+0 0.00E+0
RSF [MJ] 0.00E+0 0.00E+0 0.00E+0 0.00E+0 0.00E+0 0.00E+0 0.00E+0 0.00E+0 0.00E+0 0.00E+0
NRSF [MJ] 0.00E+0 0.00E+0 0.00E+0 0.00E+0 0.00E+0 0.00E+0 0.00E+0 0.00E+0 0.00E+0 0.00E+0
FW [m³] 4.22E-2 6.69E-5 1.01E-3 1.92E-5 0.00E+0 0.00E+0 1.05E-2 5.11E-4 -1.40E-2 -2.67E-4
PERE = Use of renewable primary energy excluding renewable primary energy resources used as raw materials; PERM = Use of
renewable primary energy resources used as raw materials; PERT = Total use of renewable primary energy resources; PENRE = Use of
non-renewable primary energy excluding non-renewable primary energy resources used as raw materials; PENRM = Use of non-
Caption
renewable primary energy resources used as raw materials; PENRT = Total use of non-renewable primary energy resources; SM = Use
of secondary material; RSF = Use of renewable secondary fuels; NRSF = Use of non-renewable secondary fuels; FW = Use of net fresh
water
RESULTS OF THE LCA – WASTE CATEGORIES AND OUTPUT FLOWS according to EN 15804+A1:
1 m² RFM average thick panel
Parameter Unit A1-A3 A4 A5 C2 C3/1 C3/2 C4/1 C4/2 D/1 D/2
HWD [kg] 9.97E-6 3.50E-8 2.01E-7 1.01E-8 0.00E+0 0.00E+0 2.04E-9 1.07E-8 -2.28E-8 -1.36E-9
NHWD [kg] 2.14E-1 4.09E-5 6.03E-2 1.16E-5 0.00E+0 0.00E+0 3.55E-2 1.97E+0 -2.05E-2 -3.95E-4
RWD [kg] 3.25E-3 1.16E-6 7.58E-5 2.89E-7 0.00E+0 0.00E+0 2.03E-4 1.52E-4 -4.86E-3 -6.34E-5
CRU [kg] 2.55E-3 0.00E+0 5.10E-5 0.00E+0 0.00E+0 0.00E+0 0.00E+0 0.00E+0 0.00E+0 0.00E+0
MFR [kg] 0.00E+0 0.00E+0 1.76E-2 0.00E+0 0.00E+0 0.00E+0 0.00E+0 0.00E+0 0.00E+0 0.00E+0
MER [kg] 0.00E+0 0.00E+0 1.96E-2 0.00E+0 0.00E+0 0.00E+0 2.00E+0 0.00E+0 0.00E+0 0.00E+0
EEE [MJ] 0.00E+0 0.00E+0 9.57E-2 0.00E+0 0.00E+0 0.00E+0 1.41E+1 4.82E-2 0.00E+0 0.00E+0
EET [MJ] 0.00E+0 0.00E+0 2.18E-1 0.00E+0 0.00E+0 0.00E+0 7.13E+0 0.00E+0 0.00E+0 0.00E+0
HWD = Hazardous waste disposed; NHWD = Non-hazardous waste disposed; RWD = Radioactive waste disposed; CRU = Components
Caption for re-use; MFR = Materials for recycling; MER = Materials for energy recovery; EEE = Exported electrical energy; EET = Exported
thermal energy
References
Standards Determination of water vapour transmission properties.
EN 15804 EN 11925
EN 15804:2012-04+A1 2013, Sustainability of EN 11925:2010
construction works — Environmental Product Reaction to fire tests. Ignitability of products subjected
Declarations — Core rules for the product category of to direct impingement of flame. Single-flame source
construction products. test.
ISO 14025
EN ISO 14025:2011-10, Environmental labels and Further References
declarations — Type III environmental declarations —
Principles and procedures. BNB
Bewertungssystem Nachhaltiges Bauen (en:
IBU 2016 assessment system sustainable building)
Institut Bauen und Umwelt e.V.: General Programme https://www.bbsr.bund.de/BBSR/EN/RP/FutureBuilding
Instructions for the Preparation of EPDs at the Institut /2SustainableBuildingQuality/2009/ServiceLife/01_Star
Bauen und Umwelt e.V. Version 1., Berlin: Institut t_dossier.html?nn=391866&notFirst=true&docId=3909
Bauen und Umwelt e.V., 2016. 00
www.ibu-epd.com
Candidate List
ISO 9001 https://echa.europa.eu/it/candidate-list-table (date
ISO 9001:2015 Quality management 27.11.2020)
ISO 14001 Clima 2019
ISO 14001: 2015 Environmental management Clima 2019 PaperPolyurethane
systems “Environmental Impacts for a Polyurethane Panel”
E. Guolo, F. Cappelletti, P. Romagnoni, F. Raggiotto
ISO 45001
ISO 45001: 2018 Occupational health and safety GaBi 9 2020
management systems GaBi 9: Documentation of GaBi 8: Software-System
and Database for Life Cycle Engineering. Copyright,
EN 13165 TM. Stuttgart, Leinfelden-Echterdingen, 1992-2020
EN 13165:2012+A2:2016 Thermal insulation products http://www.gabi-software.com
for buildings -
Factory made rigid polyurethane foam (PU) products - PANGPP 2017
Specification Piano d’ Azione Nazionale sul Green Public
Procurement (PANGPP) – Gazzetta Ufficiale della
EN 826 Repubblica Italiana, Serie Generale n.17, 11-10-2017,
EN 826:2013 Determination of Compression Behavior http://www.minambiente.it/sites/default/files/archivio/all
of Thermal Insulation Products egati/GPP/GPP_CAM_Edilizia.pdf
EN 1607 PCR Part A
EN 1607: 2013 Thermal insulating products for Product Category Rules for Building-Related Products
building applications. Determination of tensile strength and Services.
perpendicular to faces Part A: Calculation Rules for the Life Cycle
Assessment and Requirements on the Background
EN 12087 Report. Version 06.2017.
EN 12087:2013
Thermal insulating products for building applications. PCR Part B
Determination of long term water absorption by PCR Guidance-Texts for Building-Related Products
immersion. and Services; Part B: Requirements on the EPD for
Insulating materials made of foam plastics; Institute
EN 1609 Construction and Environment e.V. (IBU). Version
EN 1609: 06.2017
Thermal insulating products for building applications. https://epd-online.com
Determination of short term water absorption by partial
immersion. REACH
REACH Registration, Evaluation, Authorization and
EN 12086 Restriction of Chemical, 2007
EN 12086: 2013
Thermal insulating products for building applications.
7 Environmental Product Declaration Isolparma srl – Isolparma RFM
Publisher
Institut Bauen und Umwelt e.V. Tel +49 (0)30 3087748- 0
Panoramastr. 1 Fax +49 (0)30 3087748- 29
10178 Berlin Mail info@ibu-epd.com
Germany Web www.ibu-epd.com
Programme holder
Institut Bauen und Umwelt e.V. Tel +49 (0)30 - 3087748- 0
Panoramastr 1 Fax +49 (0)30 – 3087748 - 29
10178 Berlin Mail info@ibu-epd.com
Germany Web www.ibu-epd.com
Author of the Life Cycle
Assessment Tel +39 0544 467132
thinkstep Italy Fax +39 0544 501464
Via Bovini 43 Mail info@thinkstep.com
48123 Ravenna Web www.thinkstep.com
Italy
Owner of the Declaration
Isolparma srl Tel 049 9126213
Piazza Luigi da Porto 14 Fax 049 9129616
35131 Padova Mail info@isolparma.it
Italy Web www.isolparma.it
