ENVIRONMENTAL PRODUCT DECLARATION
as per ISO 14025 and EN 15804+A2
Owner of the Declaration Kuraray Europe GmbH
Publisher Institut Bauen und Umwelt e.V. (IBU)
Programme holder Institut Bauen und Umwelt e.V. (IBU)
Declaration number EPD-KUR-20230072-CCI1-EN
Issue date 12.05.2023
Valid to 11.05.2028
PVB film (Trosifol®)
Kuraray Europe GmbH
www.ibu-epd.com | https://epd-online.com
General Information
Kuraray Europe GmbH PVB film (Trosifol®)
Programme holder Owner of the declaration
IBU – Institut Bauen und Umwelt e.V. Kuraray Europe GmbH
Hegelplatz 1 Philipp-Reis-Str. 4
10117 Berlin 65795 Hattersheim
Germany Germany
Declaration number Declared product / declared unit
EPD-KUR-20230072-CCI1-EN Trosifol® PVB.
The declared unit is 1 m².
This declaration is based on the product category rules: Scope:
Plate glass for construction and interlayers, 01.08.2021 Trosifol PVB, manufactured in Troisdorf based on Mowital® resin from
(PCR checked and approved by the SVR) Frankfurt.
The owner of the declaration shall be liable for the underlying information
and evidence; the IBU shall not be liable with respect to manufacturer
Issue date information, life cycle assessment data and evidences.
12.05.2023
The EPD was created according to the specifications of EN 15804+A2. In
the following, the standard will be simplified as EN 15804.
Valid to
Verification
11.05.2028
The standard EN 15804 serves as the core PCR
Independent verification of the declaration and data according to ISO
14025:2011
internally X externally
Dipl.-Ing. Hans Peters
(Chairman of Institut Bauen und Umwelt e.V.)
Florian Pronold Dr. Matthew Fishwick,
(Managing Director Institut Bauen und Umwelt e.V.) (Independent verifier)
1 Environmental Product Declaration - Kuraray Europe GmbH - PVB film (Trosifol®)
Product
Constructional data
Product description/Product definition
Kuraray's polyvinyl butyral (PVB) thermoplastic films are tough, Name Value Unit
resilient safety interlayers used in laminated architectural safety Refractive index acc. to DIN EN ISO 489 1.48 -
glass. These Trosifol® PVB interlayers offer safety advantages Thermal conductivity acc. to DIN EN 993-15 0.21 W/(mK)
by retaining dangerous shards in case of glass breakage. They Thermal expansion coefficient acc. to ISO
are commonly used as safety glass interlayers available 11359-2 0.00017 K-1
worldwide.
Specific heat capacity 1.9 kJ/kgK
Surface resistivity acc. to DIN 53482 1E+13 Ω
This EPD covers all Trosifol® PVB products produced in
Troisdorf based on Mowital® resin produced in Frankfurt. Tensile strength acc. to ISO 527-3 20 N/mm2
Product codes Trosifol® B2XX and Trosifol B8XX. Elongation at break acc. to ISO 527-3 250 %
Tg acc. to DMA, 3K/min, 1Hz 32 °C
For the use and application of the product, the respective
Performance data of the product with respect to its
national provisions at the place of use apply, in Germany, for
characteristics in accordance with the relevant technical
example, the building codes of the federal states and the
provision (no CE-marking).
corresponding national specifications.
Base materials/Ancillary materials
Application
The main constituents of Trosifol® PVB film are (in mass
Trosifol® PVB film needs to be laminated between two pieces
percentages):
of glass. This sandwich arrangement is called laminated safety
-PVB resin ~72 %
glass according to EN ISO 14449. Special Trosifol® PVB
-Plasticizer ~27-28 %
grades offer additional decorative, acoustic, UV managing and
-Additives and water <1 %
structural properties.
1) This product contains substances listed in the candidate list
Technical Data
(date: 17.01.2023) exceeding 0.1 percentage by mass: no
For calculating the light, solar and heat parameters of glazing
specifically containing films from the Trosifol® & SentryGlas®
2) This product contains other Carcinogenic, Mutagenic,
product range, please go to:
Reprotoxic (CMR) substances in categories 1A or 1B which are
not on the candidate list, exceeding 0.1 percentage by mass:
https://www.trosifol.com/winslt-tool/
no
Sound Control data can be found here:
3) Biocide products were added to this construction product or it
has been treated with biocide products (this then concerns a
https://www.trosifol.com/soundlab-ai/
treated product as defined by the (EU) Ordinance on Biocide
Products No. 528/2012): no
The following data are valid for Trosifol® Clear / Trosifol®
UltraClear. Other product's data can be found in our laminator Reference service life
brochure: The reference service life is typically determined by the glass
and not by the interlayer.
https://www.trosifol.com/de/salessupport/downloads/produktbro
schueren/
LCA: Calculation rules
products and energy, as well as waste processing up to the
Declared Unit end-of-waste state or disposal of final residues during the
This declaration refers to the declared unit of 1 m2 of PVB film product stage.
(Trosifol®). The grammage of the PVB film is 0.775 kg/m2.
These modules consider the manufacturing of system
Declared unit - PVB film (Trosifol®)
components/raw materials, the transport to the production site
Name Value Unit
and the production processes of the products under study. The
Declared unit 1 m2 impact of packaging materials is included.
Grammage 0.775 kg/m2
Module A5:
Layer thickness 0.00076 m
Treatment and disposal of packaging material. Credits for
Density 1.07 g/cm3
potential avoided burdens due to energy substitution of
electricity and thermal energy generation are declared in
System boundary module D and affect only the rate of primary material (no
The type of EPD is cradle-to-gate with options, modules C1– secondary materials).
C4, and module D (A1–A3, C, D and additional module A5). In
the following section, a detailed description of the specific Module C1 to C4:
system boundaries is given: The end-of-life scenarios are as follows:
• C1 - Deconstruction/demolition: Dismantling is manual
Module A1 to A3:
(no environmental burden).
The product stage includes the provision of all materials,
2 Environmental Product Declaration - Kuraray Europe GmbH - PVB film (Trosifol®)
• C2 - Transport to treatment/disposal site: Average Land or region, in which the declared product system is
transport distance from the demolition site to waste manufactured, used or handled at the end of the product´s
treatment is assumed as 50 km to the landfill. lifespan: Europe
• C3 - Waste processing for reuse, recovery or recycling:
No waste processing (no environmental burden).
• C4 - Disposal: PVB film is 100 % landfilled. Comparability
Module D: Basically, a comparison or an evaluation of EPD data is only
For the thermal and electrical energy generated in Module A5 possible if all the data sets to be compared were created
due to the thermal treatment of packaging and product waste, according to EN 15804 and the building context, respectively
avoided burdens have been calculated by the inversion of the the product-specific characteristics of performance, are taken
electricity grid mix and thermal energy from natural gas, using into account. Background datasets: GaBi ts 10.6 software
European datasets. system and GaBi Professional 2022.1 LCI database.
Geographic Representativeness
LCA: Scenarios and additional technical information
End of life (C1-C4)
Characteristic product properties of biogenic carbon The end-of-life scenarios are as follows:
Biogenic carbon is only present in the packaging (wooden C1 - The deconstruction of the PVB film is assumed to be done
pallets and cartons). manually. Therefore, no environmental loads for the dismantling
Assumed water content in wooden pallets (packaging): 18 %. of this product are considered.
Assumed carbon content: dry wood mass consists of 50 % C2 - Transport to treatment/disposal site: Average transport
biogenic carbon and paper/cardboard 43 %. distance from the demolition site to waste treatment is assumed
as 50 km to landfill.
The biogenic carbon content of the packaging is thus: 0.129 kg C4 - Disposal: The PVB film is 100 % landfilled.
pallet/declared unit * 0.82 * 0.5 kg C / kg pallet (abs. dry) + Name ValueUnit
0.082 kg *0.43 kg C/kg cardboard= 0.08815 kg C/declared unit.
Collected as mixed construction waste [PVB film
0.775 kg
Information on describing the biogenic Carbon Content at per FU]
factory gate Landfilling [PVB film per FU] 0.775 kg
Name Value Unit
Biogenic carbon content in accompanying 0.08815 kg Reuse, recovery and/or recycling potentials (D), relevant
packaging C scenario information
The following technical scenario information is required for the For the thermal and electrical energy generated in Module A5
declared modules. due to the thermal treatment of packaging, avoided burdens
have been calculated by the inversion of the electricity grid mix
Installation into the building (A5)
and thermal energy from natural gas, using European datasets.
The packaging material treatment and disposal are also
considered in module A5.
Name Value Unit
Output substances following waste treatment on
0.2301 kg
site [packaging materials per FU]
3 Environmental Product Declaration - Kuraray Europe GmbH - PVB film (Trosifol®)
LCA: Results
DESCRIPTION OF THE SYSTEM BOUNDARY (X = INCLUDED IN LCA; ND = MODULE OR INDICATOR NOT DECLARED; MNR =
MODULE NOT RELEVANT)
Benefits and
Construction loads beyond
Product stage Use stage End of life stage
process stage the system
boundaries
la ire ta m w a Ry lp p u s tro p s n a rT g n iru tc a fu n a M e h t m o rf tro p s n a rTe tis e h t o t e ta g y lb m e s s A e s U e c n a n e tn ia M ria p e R tn e m e c a lp e R tn e m h s ib ru fe R y g re n e la n o ita re p Oe s u re ta w la n o ita re p Oe s u n o itc u rts n o c -e Dn o itilo m e d tro p s n a rT g n is s e c o rp e ts a W la s o p s iD -e s u e R-y re v o c e R-g n ilc y c e Rla itn e to p
A1 A2 A3 A4 A5 B1 B2 B3 B4 B5 B6 B7 C1 C2 C3 C4 D
X X X MND X MND MND MNR MNR MNR MND MND X X X X X
RESULTS OF THE LCA - ENVIRONMENTAL IMPACT according to EN 15804+A2: 1 m² PVB film (Trosifol®)
Parameter Unit A1-A3 A5 C1 C2 C3 C4 D
GWP-total kg CO 2 eq 3.26E+00 3.77E-01 0 2.37E-03 0 5.49E-02 -1.19E-01
GWP-fossil kg CO 2 eq 3.55E+00 5.77E-02 0 2.37E-03 0 5.49E-02 -1.18E-01
GWP-biogenic kg CO 2 eq -2.95E-01 3.2E-01 0 0 0 0 -6.05E-04
GWP-luluc kg CO 2 eq 5.4E-04 5.85E-06 0 9.09E-06 0 2.67E-05 -1.3E-05
ODP kg CFC11 eq 1.91E-09 5.63E-14 0 4.84E-16 0 7.38E-14 -7.99E-13
AP mol H+ eq 4.67E-03 7.13E-05 0 7.48E-06 0 1.63E-04 -1.56E-04
EP-freshwater kg P eq 2.99E-05 1.62E-08 0 4.71E-09 0 1.03E-05 -1.63E-07
EP-marine kg N eq 1.47E-03 2.45E-05 0 3.5E-06 0 3.6E-05 -4.22E-05
EP-terrestrial mol N eq 1.64E-02 3.28E-04 0 3.9E-05 0 3.95E-04 -4.52E-04
kg NMVOC
POCP 5.78E-03 6.56E-05 0 6.82E-06 0 1.16E-04 -1.18E-04
eq
ADPE kg Sb eq 1.61E-06 1.45E-09 0 2.36E-10 0 3.81E-09 -1.78E-08
ADPF MJ 7.95E+01 1.39E-01 0 3.13E-02 0 7.79E-01 -2.01E+00
m3 world eq
WDP -7.12E-01 3.87E-02 0 1.01E-05 0 -5.42E-04 -1.26E-02
deprived
GWP = Global warming potential; ODP = Depletion potential of the stratospheric ozone layer; AP = Acidification potential of land and water; EP =
Eutrophication potential; POCP = Formation potential of tropospheric ozone photochemical oxidants; ADPE = Abiotic depletion potential for non-fossil
resources; ADPF = Abiotic depletion potential for fossil resources; WDP = Water (user) deprivation potential)
RESULTS OF THE LCA - INDICATORS TO DESCRIBE RESOURCE USE according to EN 15804+A2: 1 m² PVB film (Trosifol®)
Parameter Unit A1-A3 A5 C1 C2 C3 C4 D
PERE MJ 1.03E+01 3.42E+00 0 2.06E-03 0 6.41E-02 -5.52E-01
PERM MJ 3.39E+00 -3.39E+00 0 0 0 0 0
PERT MJ 1.37E+01 3.22E-02 0 2.06E-03 0 6.41E-02 -5.52E-01
PENRE MJ 5.47E+01 6.94E-01 0 3.13E-02 0 2.5E+01 -2.01E+00
PENRM MJ 2.48E+01 -5.55E-01 0 0 0 -2.43E+01 0
PENRT MJ 7.96E+01 1.39E-01 0 3.13E-02 0 7.8E-01 -2.01E+00
SM kg 0 0 0 0 0 0 0
RSF MJ 0 0 0 0 0 0 0
NRSF MJ 0 0 0 0 0 0 0
FW m3 1.64E-02 9.16E-04 0 1.6E-06 0 1.01E-05 -5.31E-04
PERE = Use of renewable primary energy excluding renewable primary energy resources used as raw materials; PERM = Use of renewable primary
energy resources used as raw materials; PERT = Total use of renewable primary energy resources; PENRE = Use of non-renewable primary energy
excluding non-renewable primary energy resources used as raw materials; PENRM = Use of non-renewable primary energy resources used as raw
materials; PENRT = Total use of non-renewable primary energy resources; SM = Use of secondary material; RSF = Use of renewable secondary fuels;
NRSF = Use of non-renewable secondary fuels; FW = Use of net fresh water
RESULTS OF THE LCA – WASTE CATEGORIES AND OUTPUT FLOWS according to EN 15804+A2:
1 m² PVB film (Trosifol®)
Parameter Unit A1-A3 A5 C1 C2 C3 C4 D
HWD kg 8.63E-08 1.17E-11 0 1.37E-13 0 1.2E-10 -2.73E-10
NHWD kg 3.89E-02 2.29E-02 0 5.1E-06 0 7.72E-01 -1.02E-03
RWD kg 7.58E-04 6.07E-06 0 3.94E-08 0 9.58E-06 -1.58E-04
CRU kg 0 0 0 0 0 0 0
MFR kg 0 0 0 0 0 0 0
MER kg 0 0 0 0 0 0 0
EEE MJ 0 5.32E-01 0 0 0 0 0
EET MJ 0 9.58E-01 0 0 0 0 0
4 Environmental Product Declaration - Kuraray Europe GmbH - PVB film (Trosifol®)
HWD = Hazardous waste disposed; NHWD = Non-hazardous waste disposed; RWD = Radioactive waste disposed; CRU = Components for re-use;
MFR = Materials for recycling; MER = Materials for energy recovery; EEE = Exported electrical energy; EET = Exported thermal energy
RESULTS OF THE LCA – additional impact categories according to EN 15804+A2-optional:
1 m² PVB film (Trosifol®)
Parameter Unit A1-A3 A5 C1 C2 C3 C4 D
Disease
PM 6.26E-08 5.26E-10 0 4.26E-11 0 1.56E-09 -1.29E-09
incidence
IR kBq U235 eq 7.89E-02 9.02E-04 0 4E-06 0 1.41E-03 -2.68E-02
ETP-fw CTUe 6.53E+01 8.63E-02 0 2.4E-02 0 7.63E-01 -4.41E-01
HTP-c CTUh 9.32E-09 4.13E-12 0 4.81E-13 0 3.42E-11 -2.03E-11
HTP-nc CTUh 4.94E-08 2.79E-10 0 2.77E-11 0 2.87E-09 -7.8E-10
SQP SQP 4.91E+01 3.71E-02 0 9.38E-03 0 5.61E-02 -3.59E-01
PM = Potential incidence of disease due to PM emissions; IR = Potential Human exposure efficiency relative to U235; ETP-fw = Potential comparative
Toxic Unit for ecosystems; HTP-c = Potential comparative Toxic Unit for humans (cancerogenic); HTP-nc = Potential comparative Toxic Unit for humans
(not cancerogenic); SQP = Potential soil quality index
Disclaimer 1 – for the indicator "Potential Human exposure efficiency relative to U235". This impact category deals mainly with the
eventual impact of low-dose ionizing radiation on human health of the nuclear fuel cycle. It does not consider effects due to possible
nuclear accidents, occupational exposure or radioactive waste disposal in underground facilities. Potential ionizing radiation from the
soil, radon and from some construction materials is also not measured by this indicator.
Disclaimer 2 – for the indicators 'abiotic depletion potential for non-fossil resources', 'abiotic depletion potential for fossil resources',
'water (user) deprivation potential, deprivation-weighted water consumption', 'potential comparative toxic unit for ecosystems', 'potential
comparative toxic unit for humans – cancerogenic', 'Potential comparative toxic unit for humans - not cancerogenic', 'potential soil
quality index'. The results of this environmental impact indicator shall be used with care as the uncertainties on these results are high
as there is limited experience with the indicator.
References
Standards EN ISO 14025:2011, Environmental labels and declarations —
Type III environmental declarations — Principles and
DIN 53482 procedures.
DIN 53482:1967-01, Testing of Insulating Materials;
Determination of Electrical Resistances Values. Further References
DIN EN ISO 489 Candidate list
DIN EN ISO 489:1999-08, Plastics - Determination of the Candidate List of substances of very high concern for
refractive index (ISO 489:1999). Authorisation, published on ECHA website, latest version
17.01.2023 (https://echa.europa.eu/candidatelist-table)
DIN EN 993-15
DIN EN 993-15:2005-07, Methods of test for dense shaped GaBi
refractory products - Part 15: Determination of thermal GaBi Software System and Database for Life Cycle
conductivity by the hot-wire (parallel) method. Engineering, 1992-2021, Sphera Solutions GmbH, Leinfelden-
Echterdingen, with acknowledgement of LBP University of
DIN EN ISO 527-3 Stuttgart, program version GaBi 10; database version 2022.1.
DIN EN ISO 527-3:2019-02, Plastics - Determination of tensile
properties - Part 3: Test conditions for films and sheets (ISO GaBi documentation
527-3:2018). GaBi dataset documentation for the software system and
databases, LBP, University of Stuttgart and Sphera Solutions
EN 15804 GmbH, Leinfelden-Echterdingen, 2021. (http://www.gabi-
EN15804:2012+A1:2013, Sustainability of construction works software.com/support/gabi/gabi[1]database-2021-lci-
— Environmental Product Declarations — Core rules for the documentation/)
product category of construction products.
IBU 2021
EN 15804 Institut Bauen und Umwelt e.V.: General Instructions for the
EN 15804:2012+A2:2019+AC:2021, Sustainability of EPD programme of Institut Bauen und Umwelt e.V., Version
construction works — Environmental Product Declarations — 2.0, Berlin: Institut Bauen und Umwelt e.V., 2021 HYPERLINK
Core rules for the product category of construction products. "http://www.ibu-epd." www.ibu-epd.com
EN ISO 14449 Ordinance on Biocide Products No. 528/2012
EN 14449:2005/AC:2005, Glass in building - Laminated glass Regulation (EU) No 528/2012 of the European Parliament and
and laminated safety glass - Evaluation of conformity/Product of the Council of 22 May 2012 concerning the making available
standard. on the market and use of biocidal products
ISO 11359-2 PCR Part A
ISO 11359-2:2021-11, Plastics - Thermomechanical analysis PCR Part A: Calculation rules for the Life Cycle Assessment
(TMA) - Part 2: Determination of coefficient of linear thermal and Requirements on the Background Report according to EN
expansion and glass transition temperature. 15 804+A2:2019, Version 1.3, Institut Bauen und Umwelt e.V.,
2020.
ISO 14025
5 Environmental Product Declaration - Kuraray Europe GmbH - PVB film (Trosifol®)
PCR Part B Requirements on the EPD for plate glass for construction and
Product Category Rules for Building Products, Part B: interlayers, version 1.6, 2022 www.bau-umwelt.de
6 Environmental Product Declaration - Kuraray Europe GmbH - PVB film (Trosifol®)
Publisher
Institut Bauen und Umwelt e.V. +49 (0)30 3087748- 0
Hegelplatz 1 info@ibu-epd.com
10117 Berlin www.ibu-epd.com
Germany
Programme holder
Institut Bauen und Umwelt e.V. +49 (0)30 3087748- 0
Hegelplatz 1 info@ibu-epd.com
10117 Berlin www.ibu-epd.com
Germany
Author of the Life Cycle Assessment
Sphera Solutions GmbH +49 711 341817-0
Hauptstraße 111- 113 info@sphera.com
70771 Leinfelden-Echterdingen www.sphera.com
Germany
Owner of the Declaration
Kuraray Europe GmbH +49 69 305 85 300
Philipp-Reis-Str. 4 trosifol@kuraray.com
65795 Hattersheim https://www.kuraray.eu/
Germany
7 Environmental Product Declaration - Kuraray Europe GmbH - PVB film (Trosifol®)
