ENVIRONMENTAL PRODUCT DECLARATION
as per ISO 14025 and EN 15804+A2
Owner of the Declaration dormakaba International Holding GmbH
Publisher Institut Bauen und Umwelt e.V. (IBU)
Programme holder Institut Bauen und Umwelt e.V. (IBU)
Declaration number EPD-DOR-20210203-CBC1-EN
Issue date 19.01.2022
Valid to 18.01.2027
Ladder Pull TG138 Series
dormakaba
www.ibu-epd.com | https://epd-online.com
General Information
dormakaba Ladder Pull TG138 Series
Programme holder Owner of the declaration
IBU – Institut Bauen und Umwelt e.V. dormakaba International Holding GmbH
Hegelplatz 1 DORMA Platz 1
10117 Berlin 58256 Ennepetal
Germany Germany
Declaration number Declared product / declared unit
EPD-DOR-20210203-CBC1-EN 1 piece of the product: Ladder Pull TG138
This declaration is based on the product category rules: Scope:
Building Hardware products, 01.08.2021 This EPD refers to a specific product manufactured by dormakaba. The
(PCR checked and approved by the SVR) production site is located in Reamstown (USA).
The data represents the dormakaba financial year 2020/21.
Issue date The owner of the declaration shall be liable for the underlying information
and evidence; the IBU shall not be liable with respect to manufacturer
19.01.2022
information, life cycle assessment data and evidences.
The EPD was created according to the specifications of EN 15804+A2. In
Valid to
the following, the standard will be simplified as EN 15804.
18.01.2027
Verification
The standard EN 15804 serves as the core PCR
Independent verification of the declaration and data according to ISO
14025:2011
internally X externally
Dipl.-Ing. Hans Peters
(Chairman of Institut Bauen und Umwelt e.V.)
Florian Pronold Dr.-Ing. Wolfram Trinius,
(Managing Director Institut Bauen und Umwelt e.V.) (Independent verifier)
1 Environmental Product Declaration - dormakaba - Ladder Pull TG138 Series
Product
• Hospitality
Product description/Product definition • Entertainment
dormakaba offers a wide selection of pulls and handles for both • Education
tempered glass doors and solid material doors made of
aluminum, wood, or mixed material: Locking and non-locking Technical Data
ladder pulls, back-to-back pulls, customized handle solutions,
• Available in numerous designs and sizes
and a variety of finished materials. This EPD refers to the
• Made of 316 stainless steel
locking and non-locking ladder pull TG138 series.
• Door thicknesses up to 2-1/4' thick
For elegant and secure glass entrances, dormakaba offers the
The product with respect to its characteristics are in accordance
locking and non-locking ladder pulls — a pair of tubular
with the relevant technical provisions (no CE-marking):
lockable pull handles with a small format interchangeable
(SFIC) cylinder on the secure side and a thumbturn on the non- • Americans with Disabilities Act (ADA)
secure side of the door. Made from stainless steel, locking
Base materials/Ancillary materials
ladder pulls are perfect for the toughest interior/exterior
The composition of the product is the following:
environments. Four stocked lengths are available: 49' (1245),
60' (1524), 72' (1829), and 84' (2134) with custom sizes
available for quote upon request.
The default cylinder is a Small Format Interchangeable Core
(SFIC). Other cylinder and keying options are available. A dust
proof strike is included. For the use and application of the
product, the respective national provisions at the place of use
apply:
The product/s include/s partial articles which contain
• ANSI/BHMA A156.3-2014 substances listed in the Candidate List of REACH Regulation
1907/2006/EC (date: 19.01.2021) exceeding 0.1 percentage by
Application
mass: No.
The archtectural pulls and handles can be used for:
Reference service life
• Entrances
The reference service life of the declared product is 10 years.
• Secure areas
This corresponds to approx.. 7,500 closing cycles per year,
and following verticals:
depending on the traffic pattern and frequency of usage.
• Commercial
• Retail
LCA: Calculation rules
— A4, transport to the building site;
Declared Unit — A5, treatment of waste packaging materials arising during
The declared unit is 1 piece of the product: Ladder Pull TG138 installation into the building.
Declared unit
End-of-life stage– Modules C1-C4 and D
Name Value Unit
The end-of-life stage includes:
Declared unit 1 piece/product
— C1, de-construction, demolition;
Weight of declared unit 6.97 kg — C2, transport to waste processing;
Conversion factor to 1 kg (kg per declared — C3, waste processing for reuse, recovery and/or recycling;
0.143 -
unit) — C4, disposal; including provision and all transport, provision
of all materials, products and related energy and water use.
System boundary
Module D (Benefits and loads beyond the system boundary)
The type of EPD is according to EN 15804: "cradle to gate with
includes:
options, modules C1–C4, and module D".
— D, recycling potentials, expressed as net impacts and
The following modules are declared: A1-A3, C, D and additional
benefits.
modules: A4 + A5
Geographic Representativeness
Production - Module A1-A3
Land or region, in which the declared product system is
The product stage includes:
manufactured, used or handled at the end of the product´s
— A1, raw material extraction, processing of secondary
lifespan: North America
material input (e.g. recycling processes),
— A2, transport to the manufacturer,
— A3, manufacturing and assembly, processing and Comparability
mechanical treatments, including provision of all materials,
Basically, a comparison or an evaluation of EPD data is only
products and energy, as well as waste processing up to the
possible if all the data sets to be compared were created
end-of waste state.
according to EN 15804 and the building context, respectively
the product-specific characteristics of performance, are taken
Construction stage - Modules A4-A5
into account. Background database: GaBi, SP40
The construction process stage includes:
2 Environmental Product Declaration - dormakaba - Ladder Pull TG138 Series
LCA: Scenarios and additional technical information
Installation into the building (A5)
Characteristic product properties of biogenic carbon
Name Value Unit
Information on describing the biogenic Carbon Content at
Waste packaging 0.5 kg
factory gate
Name ValueUnit Reference service life
Biogenic carbon content in product - kg Name Value Unit
C
Life Span according to the manufacturer 10 a
Biogenic carbon content in accompanying kg
0.18
packaging C End of life (C1-C4)
Note: 1 kg of biogenic carbon is equivalent to 44/12 kg of CO . Name Value Unit
2
Recycling 6.96 kg
Energy recovery 0.01 kg
The following technical scenario information is required for the Transportation to waste management 50 km
declared modules and optional for non-declared modules.
The product is disassembled in a recycling process.Material
Transport to the building site (A4)
recycling is then assumed for the metals. The plastic
Name Value Unit components are assumed to be incinerated with energy
Litres of fuel 0.0206 l/100km recovery. Minor proportions of residues arising from the
recycling process are landfilled (1%). Region for the End of Life
Transport distance 100 km
is: Global.
Capacity utilisation (including empty runs) 55 %
Truck transport to the construction site declared for 100 km. Reuse, recovery and/or recycling potentials (D), relevant
scenario information
If necessary, the transport distance can be adjusted at building Collection rate is 100%
level.
3 Environmental Product Declaration - dormakaba - Ladder Pull TG138 Series
LCA: Results
DESCRIPTION OF THE SYSTEM BOUNDARY (X = INCLUDED IN LCA; MND = MODULE OR INDICATOR NOT DECLARED; MNR
= MODULE NOT RELEVANT)
Benefits and
Construction loads beyond
Product stage Use stage End of life stage
process stage the system
boundaries
la ire ta m w a Ry lp p u s tro p s n a rT g n iru tc a fu n a M e h t m o rf tro p s n a rTe tis e h t o t e ta g y lb m e s s A e s U e c n a n e tn ia M ria p e R tn e m e c a lp e R tn e m h s ib ru fe R y g re n e la n o ita re p Oe s u re ta w la n o ita re p Oe s u n o itc u rts n o c -e Dn o itilo m e d tro p s n a rT g n is s e c o rp e ts a W la s o p s iD -e s u e R-y re v o c e R-g n ilc y c e Rla itn e to p
A1 A2 A3 A4 A5 B1 B2 B3 B4 B5 B6 B7 C1 C2 C3 C4 D
X X X X X MND MND MNR MNR MNR MND MND X X X X X
RESULTS OF THE LCA - ENVIRONMENTAL IMPACT according to EN 15804+A2: 1 piece ladder pull TG138
Parameter Unit A1-A3 A4 A5 C1 C2 C3 C4 D
GWP-total kg CO 2 eq 4.22E+01 6.53E-02 8.13E-01 0 3.09E-02 2.29E-02 1.53E-03 -3.01E+01
GWP-fossil kg CO 2 eq 4.29E+01 6.24E-02 1.51E-02 0 2.95E-02 2.29E-02 1.52E-03 -3.02E+01
GWP-biogenic kg CO 2 eq -7.91E-01 2.88E-03 7.98E-01 0 1.37E-03 5.33E-07 5.18E-06 1.55E-01
GWP-luluc kg CO 2 eq 8.44E-02 1.49E-06 1.04E-05 0 7.03E-07 1.29E-06 4.37E-06 -6E-02
ODP kg CFC11 eq 1.89E-11 6.59E-18 1.19E-16 0 3.12E-18 1.15E-17 5.62E-18 -6.54E-14
AP mol H+ eq 2.3E-01 6.25E-05 1.37E-04 0 2.96E-05 4.07E-06 1.09E-05 -1.36E-01
EP-freshwater kg P eq 5.61E-05 1.34E-08 2.08E-08 0 6.32E-09 1.84E-09 2.61E-09 -2.65E-05
EP-marine kg N eq 3.02E-02 1.99E-05 3.88E-05 0 9.41E-06 9.18E-07 2.8E-06 -2.12E-02
EP-terrestrial mol N eq 3.28E-01 2.21E-04 5.58E-04 0 1.05E-04 1.85E-05 3.08E-05 -2.31E-01
kg NMVOC
POCP 9.12E-02 5.62E-05 1.07E-04 0 2.66E-05 2.54E-06 8.48E-06 -6.26E-02
eq
ADPE kg Sb eq 1.62E-03 1.87E-09 1.88E-09 0 8.86E-10 1.58E-10 1.36E-10 -9.31E-04
ADPF MJ 5.4E+02 8.85E-01 2.05E-01 0 4.19E-01 1.06E-02 1.99E-02 -3.68E+02
m3 world eq
WDP 1.66E+01 1.22E-04 8.95E-02 0 5.79E-05 2.34E-03 1.59E-04 -1.25E+01
deprived
GWP = Global warming potential; ODP = Depletion potential of the stratospheric ozone layer; AP = Acidification potential of land and water; EP =
Eutrophication potential; POCP = Formation potential of tropospheric ozone photochemical oxidants; ADPE = Abiotic depletion potential for non-fossil
resources; ADPF = Abiotic depletion potential for fossil resources; WDP = Water (user) deprivation potential)
RESULTS OF THE LCA - INDICATORS TO DESCRIBE RESOURCE USE according to EN 15804+A2: 1 piece ladder pull TG138
Parameter Unit A1-A3 A4 A5 C1 C2 C3 C4 D
PERE MJ 1.25E+02 2.79E-03 6.54E+00 0 1.32E-03 2.76E-03 2.61E-03 -7.87E+01
PERM MJ 6.5E+00 0 -6.5E+00 0 0 0 0 0
PERT MJ 1.31E+02 2.79E-03 3.85E-02 0 1.32E-03 2.76E-03 2.61E-03 -7.87E+01
PENRE MJ 5.4E+02 8.86E-01 2.05E-01 0 4.19E-01 2.54E-01 1.99E-02 -3.69E+02
PENRM MJ 2.43E-01 0 0 0 0 -2.43E-01 0 0
PENRT MJ 5.41E+02 8.86E-01 2.05E-01 0 4.19E-01 1.06E-02 1.99E-02 -3.69E+02
SM kg 3.3E+00 0 0 0 0 0 0 0
RSF MJ 0 0 0 0 0 0 0 0
NRSF MJ 0 0 0 0 0 0 0 0
FW m3 6.18E-01 5.01E-06 2.1E-03 0 2.37E-06 5.6E-05 5.02E-06 -4.9E-01
PERE = Use of renewable primary energy excluding renewable primary energy resources used as raw materials; PERM = Use of renewable primary
energy resources used as raw materials; PERT = Total use of renewable primary energy resources; PENRE = Use of non-renewable primary energy
excluding non-renewable primary energy resources used as raw materials; PENRM = Use of non-renewable primary energy resources used as raw
materials; PENRT = Total use of non-renewable primary energy resources; SM = Use of secondary material; RSF = Use of renewable secondary fuels;
NRSF = Use of non-renewable secondary fuels; FW = Use of net fresh water
RESULTS OF THE LCA – WASTE CATEGORIES AND OUTPUT FLOWS according to EN 15804+A2:
1 piece ladder pull TG138
Parameter Unit A1-A3 A4 A5 C1 C2 C3 C4 D
HWD kg 2.91E-06 8.59E-11 2.48E-10 0 4.07E-11 4.04E-11 3.03E-10 8.1E-08
NHWD kg 3.99E+00 9.06E-05 1.6E-02 0 4.29E-05 2.38E-03 1E-01 -2.99E+00
RWD kg 8.03E-03 9.51E-07 1.15E-05 0 4.5E-07 3.94E-07 2.27E-07 -1.93E-03
CRU kg 0 0 0 0 0 0 0 0
MFR kg 0 0 0 0 0 6.96E+00 0 0
MER kg 0 0 0 0 0 0 0 0
EEE MJ 0 0 1.13E+00 0 0 0 0 0
EET MJ 0 0 2.04E+00 0 0 0 0 0
HWD = Hazardous waste disposed; NHWD = Non-hazardous waste disposed; RWD = Radioactive waste disposed; CRU = Components for re-use;
MFR = Materials for recycling; MER = Materials for energy recovery; EEE = Exported electrical energy; EET = Exported thermal energy
4 Environmental Product Declaration - dormakaba - Ladder Pull TG138 Series
RESULTS OF THE LCA – additional impact categories according to EN 15804+A2-optional:
1 piece ladder pull TG138
Parameter Unit A1-A3 A4 A5 C1 C2 C3 C4 D
Disease
PM 4.01E-06 3.28E-10 9.25E-10 0 1.55E-10 5.2E-11 1.35E-10 -2.74E-06
incidence
IR kBq U235 eq 7.49E-01 1.36E-04 1.79E-03 0 6.43E-05 3.55E-05 2.33E-05 -2.52E-01
ETP-fw CTUe 2.68E+02 6.27E-01 9.73E-02 0 2.97E-01 3.98E-03 1.14E-02 -1.97E+02
HTP-c CTUh 9.7E-06 1.18E-11 7.46E-12 0 5.59E-12 3.45E-13 1.69E-12 -6.37E-08
HTP-nc CTUh 7.93E-07 5.05E-10 4.66E-10 0 2.39E-10 3.49E-11 1.86E-10 -1.5E-07
SQP SQP 1.79E+02 2.27E-03 5.7E-02 0 1.08E-03 3.18E-03 4.15E-03 -5.44E+01
PM = Potential incidence of disease due to PM emissions; IR = Potential Human exposure efficiency relative to U235; ETP-fw = Potential comparative
Toxic Unit for ecosystems; HTP-c = Potential comparative Toxic Unit for humans (cancerogenic); HTP-nc = Potential comparative Toxic Unit for humans
(not cancerogenic); SQP = Potential soil quality index
Disclaimer 1 – for the indicator “Potential Human exposure efficiency relative to U235”. This impact category deals mainly with the
eventual impact of low-dose ionizing radiation on human health of the nuclear fuel cycle. It does not consider effects due to possible
nuclear accidents, occupational exposure or radioactive waste disposal in underground facilities. Potential ionizing radiation from the
soil, radon and from some construction materials is also not measured by this indicator.
Disclaimer 2 – for the indicators “abiotic depletion potential for non-fossil resources”, “abiotic depletion potential for fossil resources”,
“water (user) deprivation potential, deprivation-weighted water consumption”, “potential comparative toxic unit for ecosystems”,
“potential comparative toxic unit for humans – cancerogenic”, “Potential comparative toxic unit for humans - not cancerogenic”,
“potential soil quality index”. The results of this environmental impact indicator shall be used with care as the uncertainties on these
results are high as there is limited experience with the indicator.
References
Standards IBU 2021
Institut Bauen und Umwelt e.V.: General Instructions for the
ANSI/BHMA A156.3-2014 EPDs programme of Institut Bauen und Umwelt e.V. Version
Revision of ANSI/BHMA A156.3 – 2008 2.0., Berlin: Institut Bauen und Umwelt e.V., 2021. www.ibu-
AMERICAN NATIONAL STANDARD FOR EXIT DEVICES. epd.com.
EN 15804 GaBi ts software
EN 15804:2019+A2, Sustainability of construction works — Sphera Solutions GmbH Gabi Software System and Database
Environmental Product Declarations — Core rules for the for Life Cycle Engineering 1992-2020 Version 10.0.0.71
product category of construction products.ISO 14025DIN EN University of Stuttgart Leinfelden-Echterdingen.
ISO 14025:2011-10, Environmental labels and declarations —
Type III environmental declarations — Principles and GaBi ts documentation
procedures. GaBi life cycle inventory data documentation
(https://www.gabisoftware.com/support/gabi/gabidatabase-
ISO 14025 2020-lci-documentation/).
DIN EN ISO 14025:2011-10, Environmental labels and
declarations — Type III environmental declarations — PCR Part A
Principles and procedures. PCR – Part A: Calculation Rules for the Life Cycle Assessment
and Requirements on the Project Report according to EN
Registration, Evaluation, Authorisation and Restriction of 15804+A2:2019, Version 1.0, Institut
Chemicals (REACH) Bauen und Umwelt e.V., www.ibu-epd.com.
Regulation (EC) No 1907/2006 of the European Parliament and
of the Council on the Registration, Evaluation, Authorisation PCR Part B
and Restriction of Chemicals (REACH). PCR – Part B: Requirements on the EPD for Building
Hardware product, version 1.2, Institut Bauen und
Further References Umwelt e.V., www.ibu-epd.com, 2017.
Americans with Disabilities Act Underwriters Laboratories
https://www.ada.gov/. https://ulstandards.ul.com/.
5 Environmental Product Declaration - dormakaba - Ladder Pull TG138 Series
Publisher
Institut Bauen und Umwelt e.V. +49 (0)30 3087748- 0
Hegelplatz 1 info@ibu-epd.com
10117 Berlin www.ibu-epd.com
Germany
Programme holder
Institut Bauen und Umwelt e.V. +49 (0)30 3087748- 0
Hegelplatz 1 info@ibu-epd.com
10117 Berlin www.ibu-epd.com
Germany
Author of the Life Cycle Assessment
Sphera Solutions GmbH +49 711 341817-0
Hauptstraße 111- 113 info@sphera.com
70771 Leinfelden-Echterdingen www.sphera.com
Germany
Owner of the Declaration
dormakaba International Holding GmbH +49 2333 793-0
DORMA Platz 1 info.de@dormakaba.com
58256 Ennepetal www.dormakaba.com
Germany
6 Environmental Product Declaration - dormakaba - Ladder Pull TG138 Series
