ENVIRONMENTAL PRODUCT DECLARATION
as per ISO 14025 and EN 15804+A2
Owner of the Declaration OGRO Beschlagtechnik GmbH
Publisher Institut Bauen und Umwelt e.V. (IBU)
Programme holder Institut Bauen und Umwelt e.V. (IBU)
Declaration number EPD-OGR-20240053-CBA5-EN
Issue date 18.06.2024
Valid to 17.06.2029
Stainless steel lever and window handle CORE/PREMIUM
OGRO
www.ibu-epd.com | https://epd-online.com
General Information
OGRO Stainless steel lever and window handle
CORE/PREMIUM
Programme holder Owner of the declaration
IBU – Institut Bauen und Umwelt e.V. OGRO Beschlagtechnik GmbH
Hegelplatz 1 Donnenberger Straße 2
10117 Berlin 42553 Velbert
Germany Germany
Declaration number Declared product / declared unit
EPD­OGR­20240053­CBA5­EN The declared unit is one (1 piece) stainless steel lever handle from the
OGRO PREMIUM and CORE series, including packaging materials. The
average fitting including packaging weighs 717 g.
This declaration is based on the product category rules: Scope:
Building Hardware products, 01.08.2021 This Environmental Product Declaration refers to a specific stainless steel
(PCR checked and approved by the SVR) lever handle manufactured by OGRO. The EPD isalso representative for
stainless steel window handles. The production site is located in Velbert
(Germany).
Issue date Data represents the year 2023.
18.06.2024
The owner of the declaration shall be liable for the underlying information
and evidence; the IBU shall not be liable with respect to manufacturer
information, life cycle assessment data and evidences.
Valid to
17.06.2029 The EPD was created according to the specifications of EN 15804+A2. In
the following, the standard will be simplified as EN 15804.
Verification
The standard EN 15804 serves as the core PCR
Independent verification of the declaration and data according to ISO
14025:2011
internally X externally
Dipl.­Ing. Hans Peters
(Chairman of Institut Bauen und Umwelt e.V.)
Florian Pronold Matthias Klingler,
(Managing Director Institut Bauen und Umwelt e.V.) (Independent verifier)
1 Environmental Product Declaration ­ OGRO ­ Stainless steel lever and window handle CORE/PREMIUM
Product
• DIN 17440: Steel and steel alloys
Product description/Product definition
• EN 179: Locks and fittings
OGRO Beschlagtechnik GmbH manufactures door and window
• EN 1125: Locks and fittings
fittings made of stainless steel or aluminium for the premium
• EN 1634: Fire resistance and smoke control tests for
real estate market. This EPD declares OGRO Premium and
door and shutter assemblies
CORE lever and window handles made of stainless steel.
• EN 1906: Requirements and test methods for lever
For the placing the lever handles on the market in the
handles and knob furniture
European Union/European Free Trade Association (EU/EFTA)
• EN 13126-3: Building hardware - Hardware for windows
(with the exception of Switzerland) the following legal provisions
and door height windows
apply:
• DIN 18082, Part 1: Fire protection barriers, steel doors T
• EN 179 30-1
• DIN 18095, Parts 1 + 2: Smoke control doors
For the placing the window handles on the market in the • DIN 18255: Building hardware
European Union/European Free Trade Association (EU/EFTA) • DIN 18257: Security plates
(with the exception of Switzerland) the following legal provisions • DIN 18273: Lever handle units for fire doors and smoke
apply: control doors
• DIN 4102, Parts 5 + 18: Fire behaviour of building
• EN 13126-3 materials and building components
• DIN 18040: Construction of accessible buildings
The CE­­marking takes into account the proof of conformity with
the respective harmonized standards based on the legal Performance data of the products with respect to its
provisions above. For the application and use the respective characteristics in accordance with the relevanttechnical
national provisions apply. provision which can be applied are mentioned above.
Base materials/Ancillary materials
Application The major material composition including the packaging of the
The lever an window handles are suitable for practically all product is listed below:
applications: • Stainless steel: 56%
• Steel: 26%
Lever handles: • Paper: 14%
• For use on doors which are subject to frequent force, • Plastics: 4%
e.g. football stadiums, military barracks, schools, public
toilets The lever and window handles include partial articles which
• For extremely high­traffic areas and intensive use in contain substances listed in the Candidate List of REACH
buildings Regulation1907/2006/EC (date: 14.06.2023) exceeding 0.1
• Use in public buildings, e.g. hospitals or administrative percentage by mass: yes
buildings
• Manifold barrier­free applications • Lead (Pb): 7439­92­1 (CAS­No) is used in the steel
• Use on glass doors alloy. The concentration of lead in the alloy does not
• Use on mechanically high­strength apartment entrance exceed 0,35% (by mass).
doors with requirements incl. in accordance with DIN
18257 The Candidate List can be found on the ECHA website
• Use on panic, escape, rescue and fire safety doors address: https:echa.europa.eu/de/home.
• Use on doors with electronic access control
Reference service life
Window handles: The reference service life of the stainless steel lever handles
amount to 40 years and depends on the application and
• For use on wooden, plastic or aluminium profiles
frequency of use. For repairs or renewals, suitable spare parts
• For high­traffic areas and intensive use in buildings
are available. The lever handles are tested according to EN
• Use in public buildings, e.g. hospitals or administrative
1906, meaning they are designed to withstanda minimum of
buildings
1.000.000 cycles. The reference service life of the stainless
• Suitable for all standard window handle gears with
steel window handles amount to 20 years and depends on the
variable pin adjustment
application and frequency of use. For repairs or renewals,
• Simple operation with forces according to EN standards
suitable spareparts are available. The window handles are
Technical Data tested according to EN 13126-3, meaning they are designed to
The stainless steel lever and window handles comply with withstand a minimum of 25.0000 cycles.
following standards:
LCA: Calculation rules
Name Value Unit
Declared Unit
Declared unit 1 piece/product
The declared unit is 1 piece of the product: Stainless steel lever
Mass of declared Product without
and window handle: 0.619 kg
packaging
Packaging 0.098 kg
2 Environmental Product Declaration ­ OGRO ­ Stainless steel lever and window handle CORE/PREMIUM
Other declared units are allowed if the conversion is shown processing up to the end­of waste state or disposal of final
transparently. residues during the construction process stage.
End-of-life stage– Modules C1-C4 and D
The end­of­life stage includes:— C1, de­construction,
demolition:— C2, transport to waste processing;— C3, waste
processing for reuse, recovery and/or recycling;— C4, disposal;
System boundary
including provision and all transport, provision of all materials,
The type of EPD is according to EN 15804: "cradle to products and related energy and water use. Module D (Benefits
gate with options, modules C1–C4, and module D".The and loads beyond the system boundary) includes:— D,
following modules are declared: A1­A3, C1­C4, D and recycling potentials, expressed as net impacts and benefits.
additional modules: A4 + A5
Geographic Representativeness
Production - Module A1-A3 Land or region, in which the declared product system is
The product stage includes:— A1, raw material extraction, manufactured, used or handled at the end of the product´s
processing and mechanical treatments, processing of lifespan: Global
secondary material input (e.g. recycling processes),— A2,
transport to the manufacturer,— A3, manufacturing and
assembly including provision of all materials, products and Comparability
energy, as well as waste processing up to the end­of waste Basically, a comparison or an evaluation of EPD data is only
state. possible if all the data sets to be compared were created
according to EN 15804 and the building context, respectively
Construction stage - Modules A4-A5 the product­specific characteristics of performance, are taken
The construction process stage includes:— A4, transport to the into account.
building site;— A5, installation into the building; including Background database: GaBi ts, SP40, CUP 2020.1
provision of all materials, products and energy, as well as waste
LCA: Scenarios and additional technical information
Name ValueUnit
Characteristic product properties of biogenic carbon
Output substances following waste treatment on
0.098 kg
Information on describing the biogenic carbon content at site (packaging)
factory gate
Reference service life
Name ValueUnit
kg Name Value Unit
Biogenic carbon content in product ­
C Reference service life 40 a
Biogenic carbon content in accompanying kg
0.04 End of life (C1-C4)
packaging C
C1: The product dismantling from the building is done manually
Note: 1 kg of biogenic carbon is equivalent to 44/12 kg of CO 2. without environmental burden.
C2: Transport to waste treatment at end of life is 50 km
Name Value Unit
Collected separately waste type 0.619 kg
Transport to the building site (A4)
Recycling 0.59 kg
Name Value Unit Energy recovery 0.029 kg
Litres of fuel 0.00276 l/100km
Reuse, recovery and/or recycling potentials (D), relevant
Transport distance 100 km
scenario information
Capacity utilisation (including empty runs) 55 %
The collection rate is 100%.
Transport distance is declared for 100km by truck in order to
Name Value Unit
allow scaling to a specific point of installation.
Recycling 100 %
Installation into the building (A5)
3 Environmental Product Declaration ­ OGRO ­ Stainless steel lever and window handle CORE/PREMIUM
LCA: Results
DESCRIPTION OF THE SYSTEM BOUNDARY (X = INCLUDED IN LCA; MND = MODULE OR INDICATOR NOT DECLARED; MNR
= MODULE NOT RELEVANT)
Benefits and
Construction loads beyond
Product stage Use stage End of life stage
process stage the system
boundaries
la ire ta m w a Ry lp p u s tro p s n a rT g n iru tc a fu n a M e h t m o rf tro p s n a rTe tis e h t o t e ta g y lb m e s s A e s U e c n a n e tn ia M ria p e R tn e m e c a lp e R tn e m h s ib ru fe R y g re n e la n o ita re p Oe s u re ta w la n o ita re p Oe s u n o itc u rts n o c ­e Dn o itilo m e d tro p s n a rT g n is s e c o rp e ts a W la s o p s iD ­e s u e R­y re v o c e R­g n ilc y c e Rla itn e to p
A1 A2 A3 A4 A5 B1 B2 B3 B4 B5 B6 B7 C1 C2 C3 C4 D
X X X X X MND MND MNR MNR MNR MND MND X X X X X
RESULTS OF THE LCA - ENVIRONMENTAL IMPACT according to EN 15804+A2: 1 piece
Parameter Unit A1-A3 A4 A5 C1 C2 C3 C4 D
GWP­total kg CO 2 eq 2.9E+00 6E­03 1.39E­01 0 3E­03 7.9E­02 0 ­1.97E+00
GWP­fossil kg CO 2 eq 3.06E+00 6E­03 3E­03 0 3E­03 7.9E­02 0 ­1.98E+00
GWP­biogenic kg CO 2 eq ­1.61E­01 2.77E­04 1.35E­01 0 1.2E­04 1.84E­06 0 9E­03
GWP­luluc kg CO 2 eq 5.31E­03 1.43E­07 2.29E­06 0 6.16E­08 4.45E­06 0 ­4E­03
ODP kg CFC11 eq 1.1E­12 6.33E­19 2.5E­17 0 2.73E­19 3.97E­17 0 ­4.27E­15
AP mol H+ eq 1.48E­02 6E­06 3.89E­05 0 2.59E­06 1.4E­05 0 ­8E­03
EP­freshwater kg P eq 7.03E­06 1.28E­09 4.9E­09 0 5.54E­10 6.34E­09 0 ­1.72E­06
EP­marine kg N eq 2.26E­03 1.91E­06 1.41E­05 0 8.24E­07 3.16E­06 0 ­1E­03
EP­terrestrial mol N eq 2.3E­02 2.12E­05 1.75E­04 0 9.16E­06 6.39E­05 0 ­1.4E­02
kg NMVOC
POCP 6.72E­03 5.4E­06 3.72E­05 0 2.33E­06 8.75E­06 0 ­4E­03
eq
ADPE kg Sb eq 1.17E­04 1.8E­10 3.96E­10 0 7.76E­11 5.45E­10 0 ­5.69E­05
ADPF MJ 3.89E+01 8.5E­02 4.4E­02 0 3.7E­02 3.7E­02 0 ­2.4E+01
m3 world eq
WDP 1.02E+00 1.17E­05 1.7E­02 0 5.07E­06 8E­03 0 ­7.52E­01
deprived
GWP = Global warming potential; ODP = Depletion potential of the stratospheric ozone layer; AP = Acidification potential of land and water; EP =
Eutrophication potential; POCP = Formation potential of tropospheric ozone photochemical oxidants; ADPE = Abiotic depletion potential for non­fossil
resources; ADPF = Abiotic depletion potential for fossil resources; WDP = Water (user) deprivation potential)
RESULTS OF THE LCA - INDICATORS TO DESCRIBE RESOURCE USE according to EN 15804+A2: 1 piece
Parameter Unit A1-A3 A4 A5 C1 C2 C3 C4 D
PERE MJ 1.01E+01 2.68E­04 1.18E+00 0 1.16E­04 9E­03 0 ­4.8E+00
PERM MJ 1.18E+00 0 ­1.18E+00 0 0 0 0 0
PERT MJ 1.13E+01 2.68E­04 8E­03 0 1.16E­04 9E­03 0 ­4.8E+00
PENRE MJ 3.84E+01 8.5E­02 4.4E­02 0 3.7E­02 4.99E­01 0 ­2.41E+01
PENRM MJ 4.62E­01 0 0 0 0 ­4.62E­01 0 0
PENRT MJ 3.89E+01 8.5E­02 4.4E­02 0 3.7E­02 3.7E­02 0 ­2.41E+01
SM kg 3.06E­01 0 0 0 0 0 0 0
RSF MJ 0 0 0 0 0 0 0 0
NRSF MJ 0 0 0 0 0 0 0 0
FW m3 3.9E­02 4.81E­07 4.06E­04 0 2.08E­07 1.93E­04 0 ­2.9E­02
PERE = Use of renewable primary energy excluding renewable primary energy resources used as raw materials; PERM = Use of renewable primary
energy resources used as raw materials; PERT = Total use of renewable primary energy resources; PENRE = Use of non­renewable primary energy
excluding non­renewable primary energy resources used as raw materials; PENRM = Use of non­renewable primary energy resources used as raw
materials; PENRT = Total use of non­renewable primary energy resources; SM = Use of secondary material; RSF = Use of renewable secondary fuels;
NRSF = Use of non­renewable secondary fuels; FW = Use of net fresh water
RESULTS OF THE LCA – WASTE CATEGORIES AND OUTPUT FLOWS according to EN 15804+A2:
1 piece
Parameter Unit A1-A3 A4 A5 C1 C2 C3 C4 D
HWD kg 2.13E­07 8.25E­12 6.47E­11 0 3.56E­12 1.39E­10 0 ­1.4E­07
NHWD kg 2.45E­01 8.7E­06 4E­03 0 3.76E­06 8E­03 0 ­1.63E­01
RWD kg 6.65E­04 9.13E­08 2.31E­06 0 3.94E­08 1.36E­06 0 ­1.99E­04
CRU kg 0 0 0 0 0 0 0 0
MFR kg 0 0 0 0 0 5.88E­01 0 0
MER kg 0 0 0 0 0 0 0 0
EEE MJ 0 0 2.1E­01 0 0 1.46E­01 0 0
EET MJ 0 0 3.81E­01 0 0 3.35E­01 0 0
HWD = Hazardous waste disposed; NHWD = Non­hazardous waste disposed; RWD = Radioactive waste disposed; CRU = Components for re­use;
MFR = Materials for recycling; MER = Materials for energy recovery; EEE = Exported electrical energy; EET = Exported thermal energy
4 Environmental Product Declaration ­ OGRO ­ Stainless steel lever and window handle CORE/PREMIUM
RESULTS OF THE LCA – additional impact categories according to EN 15804+A2-optional:
1 piece
Parameter Unit A1-A3 A4 A5 C1 C2 C3 C4 D
Disease
PM 2.56E­07 3.15E­11 2.16E­10 0 1.36E­11 1.79E­10 0 ­1.67E­07
incidence
IR kBq U235 eq 6.8E­02 1.31E­05 3.57E­04 0 5.63E­06 1.22E­04 0 ­2.6E­02
ETP­fw CTUe 1.73E+01 6E­02 2.1E­02 0 2.6E­02 1.4E­02 0 ­1.18E+01
HTP­c CTUh 5.72E­07 1.13E­12 1.1E­12 0 4.89E­13 1.19E­12 0 ­3.72E­09
HTP­nc CTUh 5.37E­08 4.85E­11 4.77E­11 0 2.09E­11 1.2E­10 0 ­1.06E­08
SQP SQP 2.5E+01 2.19E­04 1.2E­02 0 9.43E­05 1.1E­02 0 ­3.35E+00
PM = Potential incidence of disease due to PM emissions; IR = Potential Human exposure efficiency relative to U235; ETP­fw = Potential comparative
Toxic Unit for ecosystems; HTP­c = Potential comparative Toxic Unit for humans (cancerogenic); HTP­nc = Potential comparative Toxic Unit for humans
(not cancerogenic); SQP = Potential soil quality index
Disclaimer 1 – for the indicator “Potential Human exposure efficiency relative to U235”. This impact category deals mainly with the
eventual impact of low­dose ionizing radiation on human health of the nuclear fuel cycle. It does not consider effects due to possible
nuclear accidents, occupational exposure or radioactive waste disposal in underground facilities. Potential ionizing radiation from the
soil, radon and from some construction materials is also not measured by this indicator.
Disclaimer 2 – for the indicators “abiotic depletion potential for non­fossil resources”, “abiotic depletion potential for fossil resources”,
“water (user) deprivation potential, deprivation­weighted water consumption”, “potential comparative toxic unit for ecosystems”,
“potential comparative toxic unit for humans – cancerogenic”, “Potential comparative toxic unit for humans ­ not cancerogenic”,
“potential soil quality index”. The results of this environmental impact indicator shall be used with care as the uncertainties on these
results are high as there is limited experience with the indicator.
This EPD was created using a software tool.
References
EN 15804
EN 15804+A2:2019+AC:2021, Sustainability of construction PCR Part B
works — Environmental Product Declarations — Core rules for PCR – Part B: Requirements on the EPD for Building Hardware
the product category of construction products product, version 1.2, Institut Bauen undUmwelt e.V., www.ibu­
epd.com, 2017
ISO 14025
DIN EN ISO 14025:2011­10, Environmental labels and EN 10088
declarations — Type III environmental declarations — EN 100088:2014: Steel and steel alloys
Principles and procedures
EN 179
ECHA EN 179:2008­04: Building hardware ­ Emergency exit devices
European Chemicals Agency: https://echa.europa.eu/de/home operated by a lever handle or push pad, for use on escape
routes ­ Requirements and test methods
REACH
Registration, Evaluation, Authorisation and Restriction of EN 1125
Chemicals (REACH), Regulation (EC) No 1907/2006 EN 1125:2008­04: Building hardware ­ Panic exit devices
operated by a horizontal bar, for use on rescue routes ­
GaBi Requirements and test methods
Sphera Solutions GmbH Gabi Software System and Database
for Life Cycle Engineering 1992­2020 Version 10.0.0.71 EN 1634
University of Stuttgart Leinfelden­Echterdingen EN 1634­1:2018­04: Fire resistance and smoke control tests for
door and shutter assemblies, openable windows and elements
GaBi ts documentation of building hardware ­ Part 1: Fire­resistance test for door and
GaBi life cycle inventory data documentation https://www.gabi­ shutter assemblies and openable windows
software.com/support/gabi/gabidatabase2020­lci­
documentation/ EN 1906
EN 1906:2012­12: Building hardware ­ Lever handles and knob
LCA-tool dormakaba furniture ­ Requirements and test methods
LCA tool IBU­DOR­202104­LT1­EN, version 1.0, 2021
Developed by Sphera Solutions GmbH EN 13126-3
EN 13126­3:2023­04: Building hardware ­ Hardware for
IBU 2021 windows and door height windows ­ Requirements and test
General Instructions for the EPD programme of Institut Bauen methods ­ Part 3: Handles, primarily for tilt and turn, Tilt­first
und Umwelt e.V. Version 2.0, Berlin: Institut Bauen und Umwelt and turn­only hardware
e.V., 2021. www.ibu­epd.com
DIN 18082
PCR Part A DIN 18082­1:T1EErl MV:1993­02­03: Fire­resistant single­leaf
PCR – Part A: Calculation Rules for the Life Cycle Assessment steel doors (T 30­1 doors) – Dimensions and requirements
and Requirements on the Project Report according to
EN15804+A2:2019, Version 1.0, 2020, Institut Bauen und DIN 18095, Parts 1 + 2
Umwelt e.V., www.ibu­epd.com DIN 18095­1:1988­10: Smoke control doors; Concepts and
5 Environmental Product Declaration ­ OGRO ­ Stainless steel lever and window handle CORE/PREMIUM
requirements DIN 18095­2:1991­03: Smoke control doors; Type
testing for durability and leakage DIN 18273
DIN 18273:2015­07: Building hardware ­ Lever handle units for
DIN 18255 fire doors and smoke control doors ­ Terms and definitions,
DIN 18255:2020­05: Building hardware ­ Door lever handles, dimensions, requirements, testing and marking
backplates and escutcheons ­ Definitions, dimensions,
requirements and marking DIN 4102
DIN 4102­1:1998­05 Fire behaviour of building materials and
DIN 18257 building components – Part 1: Building materials, concepts,
DIN 18257:2022­02: Building hardware ­ Security plates ­ requirements and tests
Definitions, measurements, requirements, marking
6 Environmental Product Declaration ­ OGRO ­ Stainless steel lever and window handle CORE/PREMIUM
Publisher
Institut Bauen und Umwelt e.V. +49 (0)30 3087748­ 0
Hegelplatz 1 info@ibu­epd.com
10117 Berlin www.ibu­epd.com
Germany
Programme holder
Institut Bauen und Umwelt e.V. +49 (0)30 3087748­ 0
Hegelplatz 1 info@ibu­epd.com
10117 Berlin www.ibu­epd.com
Germany
Author of the Life Cycle Assessment
dormakaba International Holding GmbH +49 2333 793­0
DORMA Platz 1 info.de@dormakaba.com
58256 Ennepetal www.dormakaba.com
Germany
Owner of the Declaration
OGRO Beschlagtechnik GmbH +49 (0)2053 495­0
Donnenberger Straße 2 info@ogro.de
42553 Velbert www.ogro.de
Germany
7 Environmental Product Declaration ­ OGRO ­ Stainless steel lever and window handle CORE/PREMIUM
