ENVIRONMENTAL PRODUCT DECLARATION
as per ISO 14025 and EN 15804+A2
Owner of the Declaration Decospan NV
Publisher Institut Bauen und Umwelt e.V. (IBU)
Programme holder Institut Bauen und Umwelt e.V. (IBU)
Declaration number EPD-DEC-20230149-IBA1-EN
Issue date 29/08/2023
Valid to 28/08/2028
Veneered, wood flooring with HDF carrier and cork backing (10-12
mm)
Decospan NV
www.ibu-epd.com | https://epd-online.com
1. General Information
Decospan NV Veneered, wood flooring with HDF carrier and cork
backing (10-12 mm)
Programme holder Owner of the declaration
IBU – Institut Bauen und Umwelt e.V. Decospan NV
Hegelplatz 1 Lageweg 33
10117 Berlin 8930 Menen
Germany Belgium
Declaration number Declared product / declared unit
EPD-DEC-20230149-IBA1-EN 1 m² of veneered, wood flooring with HDF carrier and cork backing (10-12
mm)
This declaration is based on the product category rules: Scope:
Solid wood products, 01/08/2021 This Environmental Product Declaration covers an average square meter
(PCR checked and approved by the SVR) of pre-lacquered, veneered, wood flooring with HDF carrier and cork
backing (10-12 mm), produced by Decospan NV in Belgium.
The owner of the declaration shall be liable for the underlying information
Issue date and evidence; the IBU shall not be liable with respect to manufacturer
information, life cycle assessment data and evidences.
29/08/2023
The EPD was created according to the specifications of EN 15804+A2. In
the following, the standard will be simplified as EN 15804.
Valid to
28/08/2028 Verification
The standard EN 15804 serves as the core PCR
Independent verification of the declaration and data according to ISO
14025:2011
internally X externally
Dipl.-Ing. Hans Peters
(Chairman of Institut Bauen und Umwelt e.V.)
Florian Pronold Dr. Matthew Fishwick,
(Managing Director Institut Bauen und Umwelt e.V.) (Independent verifier)
1 Environmental-Product Declaration - Decospan NV - Veneered, wood flooring with HDF carrier and cork backing (10-12 mm)
2. Product
Name Value Unit
2.1 Product description/Product definition
Moisture content acc. to EN 322 5-9 %
Parky is a multi-layered parquet, consisting of a wood wear
Mean density 850 kg/m³
layer, pressed onto high-density fibreboard (HDF) with a
wooden backing. Parky floors are finished with a top layer of Thickness 10-12 mm
authentic wood species, sourced from responsible forestry. The Length 868-1810 mm
thickness of the veneer top layer is 0.6 mm in order to make the Width 124-166 mm
most of the material.
Reaction to fire EN 13501-1 Cfl-s1 Class
Formaldehyde emission EN 717-1 E1 Class
The thin veneer layer of 0.6 mm is pressed on the HDF-board
according to the DSI (Double-Sided Impregnation) system. Content PCP EN 14342 < 5 ppm
During this process, the adhesive is pressed into and absorbed Slip resistance CEN/TS 15676 ≥ 45 USRV
by the wood. Thermal conductivity 0.11 W/mK
Installation method floating -
The surface finish, consisting of eight robust layers of specially
developed lacquers protects the floor from wear and tear as Performance data of the product in accordance with the
well as scratches. The wood absorbs the varnish which fuses declaration of performance with respect to its essential
with the adhesive. This results in a high-strength and scratch- characteristics according to EN 14342:2013, Wood flooring and
resistant floor and a moist and dirt-resistant surface. parquet - Characteristics, evaluation of conformity and marking.
Verification and assessment of constancy of performance are
The combination of the thin top layer, the high-density carried out according to system 3.
fibreboard and the wooden backing ensures impact resistance
2.4 Delivery status
and dimensional stability. Parky floors are equipped with a click
All products are delivered in packaging units. The following
system for easy installation.
information is specified on the box:
To cover the most important products in the Parky product • Finish
range, three different product groups are distinguished, based • Wood type
on the product composition. The environmental profile was • Box quantity [m²]
calculated for each product group. • Dimensions [mm]
Group 1: Pre-lacquered, veneered wood flooring with HDF • Number of parquet planks [pcs]
carrier (7-9 mm)
Group 2: Pre-lacquered, veneered wood flooring with HDF Group 2 includes parquet planks with various formats.
carrier and cork backing (10-12 mm) Dimensions of the declared products as delivered are within
Group3: Pre-lacquered, veneered wood flooring with HDF following ranges:
carrier (10 mm)
• Length: 1203 mm
• Width: 124 - 166 mm
This EPD applies to Group 2: pre-lacquered, veneered wood
• Thickness: 10 - 12 mm
flooring with HDF carrier and cork backing (10-12 mm).
• Box quantity: 0.97 - 2.10 m²
For the placing on the market of the product in the European 2.5 Base materials/Ancillary materials
Union/European Free Trade Association (EU/EFTA) (with the The average composition of the finished products is calculated
exception of Switzerland) Regulation (EU) No. 305/2011 (CPR) per product group. The components of group 2 are given below
applies. The product needs a declaration of performance taking in kg/m² flooring.
into consideration EN 14342:2013 Wood flooring and parquet -
• Lacquer < 2 %
Characteristics, evaluation of conformity and marking as well as
• Veneer (top layer & backing) 8 – 11 %
the CE-marking. Further specification is according to EN
• Cork 3 – 5 %
14354:2017, the European standard for wood veneer floor
• Adhesive (UF-glue) < 1.5 %
coverings, as referenced by EN 14342:2013. For the
• High-density fibreboard 82 – 86 %
application and use, the respective national provisions apply.
2.2 Application This product/article/at least one partial article contains
Parky flooring is covered by harmonised standards, EN substances listed in the candidate list (17.01.2023) exceeding
14342:2013 and EN 14354:2017. It's intended as floor covering 0.1 percentage by mass: No
for internal use in dry conditions. The provided click system is
only suitable for floating installations. Flooring without an This product/article/at least one partial article contains other
integrated cork layer should be installed on a suitable underlay. carcinogenic, mutagenic, reprotoxic (CMR) substances in
Parky flooring can be installed for both private and commercial categories 1A or 1B which are not on the candidate list,
use. The installation must be carried out in accordance with the exceeding 0.1 percentage by mass: No
installation instructions, the rules of the trade and the state of
the art. Biocide products were added to this construction product or it
has been treated with biocide products (this then concerns a
2.3 Technical Data treated product as defined by the (EU) Ordinance on Biocide
Technical specifications in accordance with the information in Products No. 528/2012): No
the declaration of performance with respect to its essential
2.6 Manufacture
characteristics according to EN 14342:2013, Wood flooring and
parquet - Characteristics, evaluation of conformity and marking. Decospan produces Parky flooring at its production site in
Belgium. The production process mainly involves assembly of
Constructional data
2 Environmental-Product Declaration - Decospan NV - Veneered, wood flooring with HDF carrier and cork backing (10-12 mm)
the above, purchased components (HDF, veneer, adhesive, Health protection measures
lacquer). Decospan strictly and fully applies applicable legislation and
also complies with all requirements for general good working
Prior to the assembly process, an extended part of the conditions, in particular, with regard to health and safety.
production is dedicated to the sorting, preparing and jointing of
the veneer. Possible hazards, related to chemicals used in production, are
covered by a yearly due diligence exercise where material
Veneer is produced by slicing a log into thin layers. This safety data sheets are collected and conformity with the
process makes optimal use of the logs because, in contrast REACH-regulation (incl. SVHC's) is evaluated.
with solid wood, there is no sawing loss. Since Decospan The health and safety manager keeps track of safe use
purchases bundles of sliced veneer, the production process in guidelines and provides appropriate personal protection
Belgium starts with a sorting process. equipment when needed. Since air extraction systems filter
Incoming veneer bundles are evaluated on various aspects: ambient air in production, personal protection equipment mainly
involves:
• Wood species
• Slicing technique • Protective clothing
• Dimensions • Safety shoes
• Quality • Hearing protection
• Gloves
After the assignment of a certain quality level, the bundles are All employees are provided with the above mentioned, suitable
cut in length and width. By using advanced technology, the protection measures.
sliced wood can be joined into veneer sheets, which are again
graded, based on their quality. A committee for prevention and protection at work is in place.
Training for personnel is carried out at regular intervals,
The next step in the production process is pressing. Adhesive is including: at the start of employment, annual recap or when
applied to both sides of the HDF -carrier, which is subsequently deemed necessary.
placed onto the wooden backing. The wooden wear layer is All of this is captured in safety procedures, prevention and
placed on top. By placing this combination of materials in the protection reports and put into practice by means of e.g. fire
press at a predefined time, temperature and pressure level, the exercises, first aid training organized by the HR- and HSE-
adhesive is pressed into and absorbed by the wood. The cork manager.
layer is applied during a second pressing cycle. After pressing,
the veneered board is trimmed to the desired dimensions and Chemical residues are sorted and collected separately. These
subjected to quality control. containers are picked up by our waste processor and
processed according to applicable disposal regulations.
Finishing of the wooden wear layer is done by applying eight
layers of specially developed lacquers. Prior to this process, the Environmental protection measures
wooden wear layer is sanded and optionally brushed. The eight Decospan is FSC® (FSC-C095327) and Program for the
layers of lacquer are cured by means of UV light. This Enforcement of Forest Certification (PEFC) certified. Both
extremely strong and matt lacquer is nearly invisible. The organisations are committed to responsible forest management
quality of the finishing process is extensively inspected. and include social aspects in their policy. Wood or wood-based
materials are responsibly sourced with one of the above-
After approval of the finishing quality, the lacquered veneered mentioned certifications or as 'Pure Wood'. All suppliers are
boards are divided into parquet planks. Dimensions of the requested to sign and comply with the Pure Wood charter and
planks depend on the collection. Each plank is provided with a thus respect and commit to Decospans core values concerning
click system, which is carefully milled to the sides. responsible forestry. Internal wood waste is incinerated with
energy recovery which is re-used in the manufacturing process.
The wooden flooring is packed in cardboard boxes and
wrapped with plastic foil. 2.8 Product processing/Installation
Before starting the installation, it is essential to read the Parky
At the end of the manufacturing process, a full quality installation instructions carefully. Parky flooring is intended for
inspection check is performed and documented according to floating installation and can easily be installed, with its click
the internal Factory Production Control (FPC) system. tongue-and-groove system. Following installation tools are
recommended:
• Parky installation kit
• Pencil
• Meter
• Hammer
• Handsaw
• Cutter
Besides the above-mentioned installation tools, Parky flooring
can be processed with all tools, suitable for solid wood. These
tools must be operated in accordance with the manufacturer's
operating instructions. Make sure that the necessary safety
precautions and protection measures (e.g. hearing protection,
respiratory mask, protective gloves, safety glasses) are applied.
Provide adequate ventilation if the processing operations
generate wood dust.
2.7 Environment and health during manufacturing Dispose of the product and packaging in accordance with
applicable, local, or national disposal regulations.
3 Environmental-Product Declaration - Decospan NV - Veneered, wood flooring with HDF carrier and cork backing (10-12 mm)
life. This also applies for unusually low or high humidity,
2.9 Packaging excessive water use, dragging heavy furniture, etc.
Parky flooring is packed in a cardboard box and wrapped with Description of the influences on the ageing of the product when
PE-foil in order to protect the product during transport and applied in accordance with the rules of technology.
storage.
Packaging material must be collected separately and disposed 2.13 Extraordinary effects
of in accordance with applicable legislation. Fire
Parky, wood veneered floor covering, with surface coating and
2.10 Condition of use with or without cork bottom layer is classified as Cfl-s1. Test
Before installation, Parky flooring should be stored in a dry and conditions: in accordance with EN 13501-1:2019. Installation
protected room with an air humidity of 40 – 60 % and a method: loose-laid on end-use substrates of wood and of
temperature between 16-21°C. Wood has, as a hygroscopic classes A1 and A2-s1,d0.
material, the ability to absorb and release moisture from the
Fire protection
surrounding environment. Changes in moisture content can
result in dimensional changes over time. This needs to be Name Value
accommodated during installation by foreseeing expansion Building material class Cfl
gaps of 1 mm per running meter, as outlined in the installation Smoke gas development s1
instructions.
2.11 Environment and health during use Water
Parky flooring has a water-resistant surface but is not able to
The use phase of Parky flooring is not in the scope of the Life
withstand prolonged exposure to water. Besides damage to the
Cycle Assessment (LCA) and resulting EPD. However,
product, no adverse consequences to the environment will
measurements of VOC emissions to indoor air are measured
occur.
and available. Parky flooring complies with following regulations
and test protocols:
Mechanical destruction
• Indoor Air Comfort GOLD®
No negative impacts on the environment are identified when
• CDPH
mechanically destroying the product. Suitable personal
• M1
protection equipment is recommended to prevent injury or
Additional and more detailed information can be provided on
health risks, caused by sharp edges, wood chips or wood dust.
request. Parky flooring does not imply any hazards to water, air
or soil when used as intended. 2.14 Re-use phase
Limited mechanical damage like scratches can be repaired
2.12 Reference service life
using the Parky Repair Pens and Parky Repair Wax. Colour
The service life in accordance with the Bundesinstitut fûr Stadt-
and lacquer pens are available to repair the floor and to protect
und Raumforschung (BBSR), table "Service lives of
it from dirt and moisture.
components for life cycle assessment according to
Bewertungssystem Nachhaltiges Bauen (BNB)", is
When your floor is severely damaged, the Parky Bulldog allows
• 40 years for wooden, multilayer parquet. you to remove and replace the damaged plank(s). More
• 15 years for wood lacquers information and instructions for use are available on www.par-
The service life is specified on an informative basis and is ky-com.
based on the warranty period Decospan specifies for the
products: At end-of-life, the product can be incinerated with energy
recovery.
2.15 Disposal
Parky flooring is classified as wood waste with EWC-code 17
02 01, according to EUROSTAT Guidance.
The product must be disposed of in accordance with applicable,
local or national disposal regulations.
The following information, related to maintenance and repair is
informative, given that module B is not declared. The product 2.16 Further information
must be installed and maintained according to the Parky
Additional information, contact details, installation and
installation and maintenance instructions.
maintenance instructions are available on www.par-ky.com
Misuse or poor maintenance will adversely affect the service
3. LCA: Calculation rules
largest since the amount of HDF can vary +/- 11 %. For group 1
3.1 Declared Unit and 3 these differences are smaller, respectively 3.82 % and
The declared unit is 1 m² of pre-lacquered, veneered wood 5.88 %.
flooring with HDF carrier between 10-12 mm. The total inputs,
Declared unit
outputs and produced m² for the period under consideration are
taken as a basis. Name Value Unit
Declared unit 1 m²
The products in this EPD represent an average in a product Gross density 850 kg/m³
group. The most important variable which leads to differences
Grammage 8.26-9.96 kg/m²
in the environmental profiles within the group is the amount of
Wood moisture at delivery 5-9 %
HDF in these products. In group 2 these differences are the
Weighted averaged thickness 10-12 mm
4 Environmental-Product Declaration - Decospan NV - Veneered, wood flooring with HDF carrier and cork backing (10-12 mm)
Decospan collected data for a full production year: 2021. gas {Europe without Switzerland}| heat production, natural gas,
More specifically: at industrial furnace >100 kW |Cut-off".
• Raw material use and transport to the production
Since the LCA is based on production information from a full
location
production year it is expected that mass and energy balance is
• Decospan contacted relevant suppliers for primary data
(in) close (proximity) to complete as no materials or processes
• Energy use
have been excluded. The cut-off criteria are well below 1 %.
• Emissions
• Production
3.5 Background data
3.2 System boundary For background processes, the ecoinvent database v3.6
(allocation cut-off) has been used.
This EPD is a cradle-to-gate with options (C1-C4, D)
3.6 Data quality
Product stage A1-A3
Data quality and validation of economic flows
Parquet consists of a high-density fibreboard to which a
Decospan collected data on the production of Parky
wooden veneer layer is applied (glued) on both sides. All the
parquet for a full production year, 2021. More specifically:
raw materials are supplied to Decospan by truck. The
application of veneer onto the baseboard is called the pressing • Raw material use and transport to the production
process. This pressing is achieved by means of pressure, location
temperature and time. The panels are then sawn, sanded and • Primary data for important products were requested
varnished. After varnishing, the boards are divided in planks from suppliers
and are provided with a click system so that they can be clipped • Energy use
into one another. The heat used in the production process is • Emissions
obtained from the incineration of part of Decospan's wood • Production waste
production waste. The proportion of the electricity demand The provided data was checked for plausibility. The quality and
covered by green electricity in the total electricity demand is representativeness are considered high.
100 %. The products in this EPD represent an average in a product
group. The most important variable which leads to differences
Transport to construction (A4) in the environmental profiles within the group is the amount of
This module is not in the scope of this EPD. HDF in these products. In group 2 these differences are the
largest since the amount of HDF can vary +/- 11 %. For group 1
Construction process (A5) and 3 these differences are smaller, respectively 3.82 % and
This module is not in the scope of this EPD. 5.88 %.
Use phase (B) For background processes, the ecoinvent database v3.6
This module is not in the scope of this EPD. However, the (allocation cut-off) has been used.
emissions to indoor air will be mentioned informatively in this
EPD. Data quality and validation of environmental inventories
Since the LCA is based on production information from a full
Demolition C1 production year it is expected that mass and energy balance is
Parquet can be removed from the building in a manual process. close to complete. For the LCA calculations, the following
It is anticipated that the environmental impact of this process is methods have been used:
neglectable. • SimaPro's LCA method: "EN 15804+A2" via
bepalingsmethode 'set 1', 'set 2' & param (NMD 3.4)
Recovery D (see appendix C)
This module includes the benefit of the recovery of electricity SGS INSTRON has checked potential uncharacterised
and heat that often occurs in waste incineration plants. For the substances. This check is part of the validation of
electrical and thermal efficiency of the waste-to-energy plant we environmental inventories.
calculated with 18 % and 31 % respectively. For the heat of
combustion of parquet (wood) the lower heating value was 3.7 Period under review
used: Wood: 13.99 MJ/kg. The production data for this EPD is based on the production of
a full production year (2021).
3.3 Estimates and assumptions
Transport to waste treatment C2 3.8 Geographic Representativeness
After the parquet is removed from the application is transported Land or region, in which the declared product system is
to a waste treatment facility. In the waste treatment scenario in manufactured, used or handled at the end of the product´s
this LCA, a transport distance of 50 km is assumed. lifespan: Belgium
3.4 Cut-off criteria
Emissions for the combustion of wood are not measured at the 3.9 Allocation
plant and are therefore included via the ecoinvent used. There The energy use for the production processes has been
is a process-specific emission to be expected from allocated based on the area produced for each of the products.
formaldehyde. The exact emission is not measured and The amount of production waste has been allocated based on
therefore included based on the ecoinvent process "Glued the mass of the products and the loss factor for each of the
laminated timber, for indoor use {RER}| production | Cut-off". products.
The emission included in the calculation is 0.0114 kg/m3
product. The avoided production of electricity from primary 3.10 Comparability
sources is based on: "Electricity, high voltage {NL}|heat and Basically, a comparison or an evaluation of EPD data is only
power co-generation, natural gas, combined cycle power plant, possible if all the data sets to be compared were created
400MWelectrical | Cut-off". The avoided production of heat from according to EN 15804 and the building context, respectively
primary sources is based on: "Heat, district or industrial, natural the product-specific characteristics of performance, are taken
5 Environmental-Product Declaration - Decospan NV - Veneered, wood flooring with HDF carrier and cork backing (10-12 mm)
into account. For background processes the ecoinvent database v3.6 (allocation cut-off) has been used.
4. LCA: Scenarios and additional technical information
Reference service life
Characteristic product properties biogenic carbon
The service life is declared in accordance with the
The amount of biogenic C in the product has been calculated
BBSR, table "Service lives of components for life cycle
using the amount of veneer, HDF and cork in the product,
assessment according to BNB".
multiplication by the wood and cardboard content and 0.5. The
latter is the amount of C in wood according to EN 16485:2014. Name Value Unit
The wood content in HDF is 77 % according to the suppliers Life Span According to BBSR 15 years
EPD: EPD-UNI-20150013-IBA1-EN. For veneer and cork, a Life span According to the See section
moisture content of 6 % has been used. manufacturer 2.12 -
Note: 1 kg of biogenic carbon is equivalent to 44/12 kg of CO2.
Information on describing the biogenic carbon content at End of life (C1-C4)
factory gate Demolition C1
Parquet is typically removed from the building in a manual
Name ValueUnit
process. It is anticipated that the environmental impact of this
kg
Biogenic carbon content in product 3.51 process is neglectable.
C
Biogenic carbon content in accompanying 0.078 kg Transport to waste treatment C2
packaging C After the parquet is removed from the application it is
transported to a waste treatment facility. In the waste treatment
Use or application of the installed product (B1) see section scenario in this LCA a transport distance of 50 km is assumed
2.12 "Use" (ecoinvent: "Transport, freight, lorry, unspecified {GLO}| market
This module is not in scope. However, the emissions to indoor group for transport, freight, lorry, unspecified | Cut-off").
air are informatively mentioned in section 2.11.
Waste processing (C3)
The following information, related to maintenance and repair is The waste treatment scenario in this study assumes that at the
informative, given that module B is not declared. waste treatment facility the parquet is chipped into wood
chips.The following ecoinvent process is used: "Wood chipping,
Maintenance (B2) industrial residualwood, stationary electric chipper {GLO}|
The specially developed Parky Wood Floor Cleaner is market for | Cut-off".
recommended to maintain the parquet. It removes dirt without
harming the lacquer. Maintenance instructions are available on Final waste treatment (C4)
www.par-ky.com The waste treatment scenario in this study assumes that the
wood chips are used for incineration with energy recovery. It is
Repair (B3) assumed that the energy efficiency of energy recovery is 18 %
Limited mechanical damage like scratches can be repaired electric and 31 % thermal. Since this efficiency is <60 %, the
using the Parky Repair Pens and Parky Repair Wax. Colour incineration process is included in module C4.
and lacquer pens are available to repair the floor and protect it Name Value Unit
from dirt and moisture. Collected separately waste wood 9.04 kg
Energy recovery 9.04 kg
Replacement (B4) / Refurbishment (B5)
When your floor is severely damaged, the Parky Bulldog allows Reuse, recovery and/or recycling potentials (D), relevant
you to remove and replace the damaged plank(s). More scenario information.
information and instructions for use are available on www.par- The benefit of the recuperation of electricity and heat that often
ky.com. occurs in waste incineration plants was included in module D.
6 Environmental-Product Declaration - Decospan NV - Veneered, wood flooring with HDF carrier and cork backing (10-12 mm)
5. LCA: Results
DESCRIPTION OF THE SYSTEM BOUNDARY (X = INCLUDED IN LCA; ND = MODULE OR INDICATOR NOT DECLARED; MNR =
MODULE NOT RELEVANT)
Benefits and
Construction loads beyond
Product stage Use stage End of life stage
process stage the system
boundaries
la ire ta m w a Ry lp p u s tro p s n a rT g n iru tc a fu n a M e h t m o rf tro p s n a rTe tis e h t o t e ta g y lb m e s s A e s U e c n a n e tn ia M ria p e R tn e m e c a lp e R tn e m h s ib ru fe R y g re n e la n o ita re p Oe s u re ta w la n o ita re p Oe s u n o itc u rts n o c -e Dn o itilo m e d tro p s n a rT g n is s e c o rp e ts a W la s o p s iD -e s u e R-y re v o c e R-g n ilc y c e Rla itn e to p
A1 A2 A3 A4 A5 B1 B2 B3 B4 B5 B6 B7 C1 C2 C3 C4 D
X X X MND MND MND MND MNR MNR MNR MND MND X X X X X
RESULTS OF THE LCA - ENVIRONMENTAL IMPACT according to EN 15804+A2: 1 m² veneered wood flooring with HDF carrier
and cork backing (10-12 mm)
Parameter Unit A1-A3 C1 C2 C3 C4 D
Global Warming Potential total (GWP-total) kg CO 2 eq -7.02E+00 0 1.26E-01 1.28E-01 1.99E+01 -6.06E-01
Global Warming Potential fossil fuels (GWP-fossil) kg CO 2 eq 1.26E+01 0 1.26E-01 1.27E-01 1.35E-01 -5.44E-01
Global Warming Potential biogenic (GWP-biogenic) kg CO 2 eq -1.98E+01 0 5.8E-05 9.95E-04 1.98E+01 -5.61E-02
Global Warming Potential luluc (GWP-luluc) kg CO 2 eq 1.74E-01 0 4.6E-05 2.28E-04 2.42E-05 -6.26E-03
Depletion potential of the stratospheric ozone layer (ODP) kg CFC11 eq 9.48E-07 0 2.77E-08 5.76E-09 1.09E-08 -1.59E-07
Acidification potential of land and water (AP) mol H+ eq 8.47E-02 0 7.29E-04 6.45E-04 1.53E-03 -1.77E-02
Eutrophication potential aquatic freshwater (EP-freshwater) kg P eq 1.74E-03 0 1.27E-06 7.74E-06 1.76E-06 -5.58E-05
Eutrophication potential aquatic marine (EP-marine) kg N eq 1.51E-02 0 2.57E-04 1.07E-04 7.2E-04 -5.18E-03
Eutrophication potential terrestrial (EP-terrestrial) mol N eq 1.71E-01 0 2.83E-03 1.22E-03 7.67E-03 -8.52E-02
Formation potential of tropospheric ozone photochemical oxidants kg NMVOC
5.7E-02 0 8.08E-04 3.29E-04 1.89E-03 -1.49E-02
(POCP) eq
Abiotic depletion potential for non fossil resources (ADPE) kg Sb eq 1.04E-04 0 3.18E-06 3.12E-07 1.75E-06 -7.99E-06
Abiotic depletion potential for fossil resources (ADPF) MJ 2.03E+02 0 1.89E+00 1.74E+00 1.19E+00 -6.54E+00
m3 world eq
Water use (WDP) 3.57E+00 0 6.78E-03 2.12E-02 -1.05E-01 -5.83E-02
deprived
RESULTS OF THE LCA - INDICATORS TO DESCRIBE RESOURCE USE according to EN 15804+A2: 1 m² veneered wood
flooring with HDF carrier and cork backing (10-12 mm)
Parameter Unit A1-A3 C1 C2 C3 C4 D
Renewable primary energy as energy carrier (PERE) MJ 3.12E+02 0 2.37E-02 2.13E-01 2.71E-02 -1.41E+02
Renewable primary energy resources as material utilization
MJ 0 0 0 0 0 0
(PERM)
Total use of renewable primary energy resources (PERT) MJ 3.12E+02 0 2.37E-02 2.13E-01 2.71E-02 -1.41E+02
Non renewable primary energy as energy carrier (PENRE) MJ 2.14E+02 0 2.01E+00 1.84E+00 1.29E+00 -6.95E+00
Non renewable primary energy as material utilization (PENRM) MJ 0 0 0 0 0 0
Total use of non renewable primary energy resources (PENRT) MJ 2.14E+02 0 2.01E+00 1.84E+00 1.29E+00 -6.95E+00
Use of secondary material (SM) kg 0 0 0 0 0 0
Use of renewable secondary fuels (RSF) MJ 0 0 0 0 0 0
Use of non renewable secondary fuels (NRSF) MJ 0 0 0 0 0 0
Use of net fresh water (FW) m3 1.2E-01 0 2.31E-04 1.03E-03 -1.98E-03 -1.74E-03
RESULTS OF THE LCA – WASTE CATEGORIES AND OUTPUT FLOWS according to EN 15804+A2:
1 m² veneered wood flooring with HDF carrier and cork backing (10-12 mm)
Parameter Unit A1-A3 C1 C2 C3 C4 D
Hazardous waste disposed (HWD) kg 2.29E-02 0 4.8E-06 7.11E-07 2.75E-06 -2.32E-05
Non hazardous waste disposed (NHWD) kg 2.22E+00 0 1.2E-01 1.16E-02 1.08E-01 -2.54E-01
Radioactive waste disposed (RWD) kg 9.95E-04 0 1.24E-05 6.7E-06 2.63E-06 -4.2E-05
Components for re-use (CRU) kg 0 0 0 0 0 0
Materials for recycling (MFR) kg 0 0 0 0 0 0
Materials for energy recovery (MER) kg 0 0 0 0 0 0
Exported electrical energy (EEE) MJ 0 0 0 0 2.34E+01 0
Exported thermal energy (EET) MJ 0 0 0 0 4.04E+01 0
RESULTS OF THE LCA – additional impact categories according to EN 15804+A2-optional:
1 m² veneered wood flooring with HDF carrier and cork backing (10-12 mm)
Parameter Unit A1-A3 C1 C2 C3 C4 D
Disease
Incidence of disease due to PM emissions (PM) 8.96E-07 0 1.13E-08 4.52E-09 1.58E-08 -2.4E-07
incidence
Human exposure efficiency relative to U235 (IR) kBq U235 eq 1.02E+00 0 7.94E-03 8.89E-03 1.95E-03 -2.74E-02
7 Environmental-Product Declaration - Decospan NV - Veneered, wood flooring with HDF carrier and cork backing (10-12 mm)
Comparative toxic unit for ecosystems (ETP-fw) CTUe 3.38E+02 0 1.69E+00 2.27E+00 2.13E+00 -1.72E+02
Comparative toxic unit for humans (carcinogenic) (HTP-c) CTUh 2.12E-08 0 5.48E-11 4.61E-11 3.77E-10 -1.97E-09
Comparative toxic unit for humans (noncarcinogenic) (HTP-nc) CTUh 1.81E-07 0 1.85E-09 1.29E-09 2.01E-08 -7.17E-08
Soil quality index (SQP) SQP 1.48E+03 0 1.64E+00 3.12E-01 3.71E-01 -6.76E+02
Disclaimer 1 – for the indicator “Potential Human exposure efficiency relative to U235”. This impact category deals mainly with the
eventual impact of low-dose ionizing radiation on human health of the nuclear fuel cycle. It does not consider effects due to possible
nuclear accidents, occupational exposure nor due to radioactive waste disposal in underground facilities. Potential ionizing radiation
from the soil, from radon and from some construction materials is also not measured by this indicator.
Disclaimer 2 – for the indicators “abiotic depletion potential for non-fossil resources”, “abiotic depletion potential for fossil resources”,
“water (user) deprivation potential, deprivation-weighted water consumption”, “potential comparative toxic unit for ecosystems”,
“potential comparative toxic unit for humans – cancerogenic”, “Potential comparative toxic unit for humans - not cancerogenic”,
“potential soil quality index”. The results of this environmental impact indicator shall be used with care as the uncertainties on these
results are high or as there is limited experienced with the indicator.
6. LCA: Interpretation
8 Environmental-Product Declaration - Decospan NV - Veneered, wood flooring with HDF carrier and cork backing (10-12 mm)
To visualize which materials and processes give the largest
contribution to the environmental indicators, a major The production of HDF gives the largest contribution to most of
contributions analysis has been included. In the graph, the total the environmental indicators. The exceptions are GWP where
value of each indicator has been set to 100 %. The colours the incineration of wood (waste) gives
indicate which part of the environmental effects are caused by the largest contribution.
the different materials and processes in the life cycle of the
parquet.
7. Requisite evidence
Use phase (B) is not in the scope of this LCA, however, the
AgBB overview of results (3 days [µg/m³])
emissions to indoor air will be mentioned informatively. VOC
Name Value Unit
emission test reports by Eurofins Product Testing A/S,
Smedeskovvej 38, 8464 Galten, Denmark are available. The TVOC (C6 - C16) 13 μg/m3
highest measured values of all objects, included in group 2, is Sum SVOC (C16 - C22) < 5 μg/m3
given.
R (dimensionless) 0.085 -
7.1. Formaldehyde
VOC without NIK < 5 μg/m3
Test method: EN 16516
Name Value Unit Carcinogenic Substances < 1 μg/m3
EN 717-1 8.3 µg/m³ Comparison with limit values of
- French VOC Regulation
- French CMR Components
- Belgian Regulation
7.2. VOC emissions
Name Value Unit
AgBB overview of results (28 days [µg/m³])
French VOC Regulation A+ -
Name Value Unit
French CMR Components Pass -
TVOC (C6 - C16) 11 μg/m3
Belgian Regulation Pass -
Sum SVOC (C16 - C22) < 5 μg/m3
R (dimensionless) 0.095 -
VOC without NIK < 5 μg/m3
Carcinogenic Substances < 1 μg/m3
8. References
Standards
EN 12667
EN 322 EN 12667:2001, Thermal performance of building materials and
EN 322:1994, Wood-based panels - Determination of moisture products - Determination of thermal resistance by means of
content guarded hot plate and heat flow meter methods - Products of
high and medium thermal resistance
EN 717-1
EN 717-1:2004, Wood-based panels - Determination of EN 13501-1
formaldehyde release - Part 1: Formaldehyde emission by the EN 13501-1:2019, Fire classification of construction products
chamber method and building elements - Part 1: Classification using data from
9 Environmental-Product Declaration - Decospan NV - Veneered, wood flooring with HDF carrier and cork backing (10-12 mm)
reaction to fire tests CDPH
Californian Department of Public Health Standard Method for
ISO 14025 VOC Emissions
ISO 14025:2006 Environmental labels and declarations — Type
III environmental declarations — Principles and procedures, ECHA Candidate List
2006. List of Substances of Very High Concern (SVHC) Candidate for
Authorisation (ECHA Candidate List), dated 17.01.2023,
ISO 14040 published in accordance with Article 59(10) of the REACH
ISO 14040:2006 Environmental management — Life cycle Regulation. Helsinki: European Chemicals Agency.
assessment — Principles and framework, 2006.
EUROSTAT
ISO 14044 European waste classification for statistics
ISO 14044:2006 Environmental management — Life cycle
assessment — Requirements and guidelines, 2006. EWC-code
EWC-code 17 02 01: Non-hazardous wood waste
EN 14342
EN 14342:2013, Wood flooring - Characteristics, evaluation of French VOC Regulation
conformity and marking Regulation of March and May 2011 (DEVL1101903D and
DEVL1104875A)
EN 14354
EN 14354: 2017, Wood veneer floor coverings French CMR Components
Regulation of April and May 2009
CEN/TS 15676
CEN/TS 15676:2007, Wood flooring, slip resistance FSC®
Forest Stewardship Council
EN 15804 License number: FSC-C095327
EN 15804:2012+A2:2019, Sustainability of construction works -
Environmental product declarations - Core rules for the product IBU 2021
category of construction products, 2019. Institut Bauen und Umwelt e.V.: General Instructions for the
EPD programme of Institut Bauen und Umwelt e.V., Version
EN 16485 2.0, Berlin: Institut Bauen und Umwelt e.V., 2021 HYPERLINK
EN 16485:2014; Round and sawn timber - Environmental "http://www.ibu-epd." www.ibu-epd.com
Product Declarations - Product category rules for wood and
wood-based products for use in construction, 2014. Indoor Air Comfort Gold®
Eurofins product certification
EN 16516
EN 16516:2017+A1:2020, Construction products: Assessment M1
of release of dangerous substances - Determination of Finnish classification test for building materials
emissions into indoor air.
PEFC
ISO 21930 Programme for the Endorsement of Forest Certification
ISO 21930:2017 Sustainability in buildings and civil engineering Schemes.
works — Core rules for environmental product declarations of License number: PEFC/07-31-60
construction products and services, 2017.
PCR Part A
Further references 'Product Category Rules for Building-Related Products and
Services Part A: Calculation Rules for the Life Cycle
AgBB/ABG Assessment and Requirements on the Project Report according
Anforderungen an bauliche Anlagen bezüglich des to EN 15804+A2:2019 Version 1.3,'
Gesundheitsschutzes (ABG)
PCR Part B
AltholzV 'Product Category Rules for Building-Related Products and
Ordinance on Requirements for the Recovery and Disposal of Services Part B: Requirements on the EPD for Solid wood
Waste Wood of 15 August 2002 (BGBl. I p. 3302), last products.'
amended by Article 120 of the Ordinance of 19 June 2020 Institut Bauen und Umwelt e.V., 2021.
(BGBl. I p. 1328).
Regulation (EU) No 305/2011
Belgian Regulation of the European Parliament and of the Council of 9 March 2011
Royal decree of May 2015 laying down harmonised conditions for the marketing of
construction products
BBSR
Bundesinstitut für Bau-, Stadt- und Raumforschung Regulation (EU) No 528/2012
of the European Parliament and the Council of 12 May 2012
BNB concerning the making available on the market and use of
BNB Code No. 352.812 Useful lives of building components for biocidal products.
life cycle analyses according to the Sustainable Building
Assessment System, 2017: Wood multilayer parquet. Berlin: Software/database
Federal Ministry of the Interior, for Construction and Home Ecoinvent database v3.6
Affairs.
10 Environmental-Product Declaration - Decospan NV - Veneered, wood flooring with HDF carrier and cork backing (10-12 mm)
11 Environmental-Product Declaration - Decospan NV - Veneered, wood flooring with HDF carrier and cork backing (10-12 mm)
Publisher
Institut Bauen und Umwelt e.V. +49 (0)30 3087748- 0
Hegelplatz 1 info@ibu-epd.com
10117 Berlin www.ibu-epd.com
Germany
Programme holder
Institut Bauen und Umwelt e.V. +49 (0)30 3087748- 0
Hegelplatz 1 info@ibu-epd.com
10117 Berlin www.ibu-epd.com
Germany
Author of the Life Cycle Assessment
SGS INTRON +31 88 214 52 04
Dr. Nolenslaan 126 nl.intron@sgs.com
6136GV Sittard www.sgs.com/intron
Netherlands
Owner of the Declaration
Decospan NV +32 (0)56 88 99 00
Lageweg 33 compliance@decospan.com
8930 Menen https://www.decospan.com/
Belgium
12 Environmental-Product Declaration - Decospan NV - Veneered, wood flooring with HDF carrier and cork backing (10-12 mm)
