Environmental Product
Declaration
as per ISO 14025 and EN 15804
Owner of the declaration: Dr. Schutz GmbH
Publisher: Kiwa-Ecobility Experts
Programme operator: Kiwa-Ecobility Experts
Registration number: EPD-Dr. Schutz-280-EN
Issue date: 16.01.2023
Valid to: 16.01.2028
Dr. Schutz® PU Color
Colored 2part polyurethane sealer, waterbased /
Farbiger 2K Polyurethansiegel auf Wasserbasis
1. General information
Dr. Schutz GmbH Dr. Schutz® PU Color
Programme operator Owner of the declaration
Kiwa-Ecobility Experts Dr. Schutz GmbH
Voltastr. 5 Holbeinstraße 17
13355 Berlin 53175 Bonn
Germany Germany
Registration number Declared product / declared unit
EPD-Dr. Schutz-280-EN 1 m2 floor sealer
This declaration is based on the Product Scope
Category Rules Dr. Schutz® PU Color is a water-based 2part-
EN 16810: 2017 - Resilient, textile and lami- polyurethane sealer for professional use. It is
nate floor coverings - Environmental product produced and distributed by Dr. Schutz GmbH,
declarations - Product category rules issue located in Bonn (Germany). The EPD refers to
2017-08 the specific product.
EPD type: Cradle to gate with modules A4, A5,
Issue date C and module D.
16.01.2023 Kiwa-Ecobility Experts shall not be liable with
respect to manufacturer information, life cy-
Valid to cle assessment data and evidence.
16.01.2028
Verification
The European standard EN 15804+A2:2019
serves as the core PCR.
Independent verification of the declaration
and data according to ISO 14025:2011-10
☐internal ☒external
Frank Huppertz
(Head of Kiwa-Ecobility Experts)
Prof. Dr. Frank Heimbecher Elisabet Amat - Greenize Projects S.L.U.
(Chairman of the independent expert committee – (Third party verifier)
Kiwa-Ecobility Experts)
Page | 2 Dr. Schutz GmbH – PU Color
2. Product
2.1 Product description
PU Color is a colored, waterbased two-part polyurethane sealer. It is a hardwearing sealer film, with
excellent elasticity and good resistance against colorless chemicals intended only for professional use.
It is available in different color shades, that can be freely chosen by the costumer from RAL-K5, NCS-S,
Pantone and Sikkens 4041 color codes.
2.2 Application
Before application, the floor needs to be cleaned and roughened. First a wet cleaning using a detergent
is carried out, followed by a neutralisation/post-cleaning with clear water. Final, roughening of the
surface is necessary, to ensure a good adhesion of the sealing. The PU Color lacquer is mixed on site
with the crosslinker in a ratio of 10:1. The mixture is then applied to the properly prepared surface,
with a coverage of 90-100 ml/m². Two layers are necessary, depending on the absorbency of the sub-
surface and the contrast, more applications may be needed until the surface is effectively covered. The
detailed application instructions can be found online (https://www.dr-schutz.com/wp-content/up-
loads/PI_EN_PU_Color_200803.pdf)
2.3 Technical data
Name Value Unit
PU Color (lacquer) Crosslinker
Physical state Fluid Fluid -
Colour Whitish Colourless -
Melting point Undetermined Undetermined °C
Boiling point >98 Undetermined °C
Flash point >100 65 °C
Auto-ignition temperature 194 165 °C
pH (at 20°C) 8.5 Not determined
Kinematic viscosity (at 20°C) 90 26 s (DIN 53211/4)
Not miscible or difficult
Solubility water Fully miscible
to mix
Vapour pressure (at 20°C) 23 Not determined hPa
Density at (20°C) 1.035 1.075 g/cm³
Organic solvents 10 29.9 %
VOC 10 29.9 %
2.3 Placing on the market/ Application rules
The product is captured under the Giscode W3DD+ / 2004/42/IIA(j)(140)140 (product group water seal
with isocyanate hardener, solvent content up to 15% ). It is defined as a good not dangerous by
transport regulations by the ADR/RID (Agreement concerning the International Carriage of Dangerous
Goods by Road/Convention concerning International Carriage by Rail).
The product is packed as a set, consisting of a 5kg PP-bucket with PU color lacquer and a 550 ml HDPE-
bottle with crosslinker, both packed in a corrugated cardboard box.
The main market area is Germany (approx. 50%), followed by neighboring countries (35%), other Eu-
ropean countries (12%) and overseas (3%).
Page | 3 Dr. Schutz GmbH – PU Color
2.4 Base materials / Ancillary materials
Dr. Schutz® PU Color is a water-based 2part-polymer-sealer, consisting of a PU Color lacquer and a
crosslinker mixed on site. The main ingredients of the lacquer are water, colorants, and different pol-
ymers, while the crosslinker is a mixture of isocyanates and glycol ethers. The ingredients divided
according to substance class are shown separately for the PU Color lacquer and the crosslinker below.
PU Color lacquer
Substance class Total value (in %)
Water 10-15
Polymer dispersion 45-55
Film forming aids 6-10
Additives (antifoaming agents, thickener, levelling agents etc.) 5-25
Crosslinker
Substance class Total value (in %)
Isocyanate 70
Glycol ether 30
The total mass of biogenic carbon containing materials is less than 5 % of the total mass of the product
and associated packaging (only the corrugated board box packaging contains biogenic carbon, having
a mass share of approx. 4% on each product), therefore the biogenic carbon content may be omitted.
The product does not contain substances included in the “Candidate list of substances of very high
concern for authorisation” (SVHC).
2.5 Manufacturing
The manufacturing is located at Dr. Schutz GmbH, Holbeinstraße 17, 53157 Bonn, Germany. The raw
materials are added together and mixed according to the recipe. For this purpose, a stirring device,
pumps, stackers, etc. are required, powered by electricity and gas.
The finished lacquer is drawn onto IBC's by free fall or pump and filled from the IBC’s into canisters by
a filling machine.
The crosslinker is produced according to the recipe at a third-party filler and filled by machine in bottles
delivered to the manufacturing site on pallets.
The manufacturing process is shown in the following figure:
Page | 4 Dr. Schutz GmbH – PU Color
Figure 1: Process flow chart of the production of Dr. Schutz® PU Color
2.6 Packaging
The canisters and bottles get labelled and for a set, one canister lacquer and one bottle crosslinker are
packed in corrugated board boxes and stacked onto pallets for further transport. The pallets are
stretched with film.
2.7 Reference Service Life (RSL)
The producer recommends a renewal of the seal every 6 years. Therefore, the reference service life of
the product is assumed to be 6 years.
2.8 Other Information
For further information on Dr. Schutz® products please visit the official webpage under the following
link: https://www.dr-schutz.com/
Page | 5 Dr. Schutz GmbH – PU Color
3. LCA: Calculation rules
3.1 Declared unit
In accordance with the PCR B 1 m2 of applied floor sealing is chosen as the declared unit. Although a
unit of mass should be used for cradle-to-gate scopes, in this case, where the application can be une-
quivocally defined, the chosen unit is a functional unit of 1 m². The PCR is intended for com-plete floor
coverings (such as resilient floors, textile floors etc.). There is no PCR available for floor sealers in par-
ticular, therefore EN 16810:2017 was chosen to be applicable for the calculated prod-ucts, which after
application can be considered to be part of the flooring. Furthermore, the declara-tion of m² as de-
clared unit as specified by the PCR is necessary and reasonable, as the installation phase should be
considered due to its high impact which is only possible in a declaration per m² and not per kg of sealer.
Product Unit Value
Declared Unit m2 floor sealing 1
Unit weight g/m2 200
3.2 System boundary
The Environmental Product Declaration is a life cycle with a functional unit. It considers all potential
environmental impacts of the product from the cradle to gate, distribution, installation and the end of
life. The manufacturing phase includes the production or extraction of the source materials, the
transport to the respective production plant and the production of the geogrids. All inputs (raw mate-
rials, pre-cursors, energy, and auxiliary materials) as well as the by-products and waste are considered
for all life cycle phases. Finally, only production-related energy consumption (excluding administration
and social rooms) is considered.
The use phase (modules B1 to B7) is not considered, as maintenance (e.g. floor cleaning or sweeping)
is highly user dependent and varies.
The year 2021 represents the time reference for raw materials and energy consumption. Due to the
production location Germany is considered as the geographical reference area. However, environmen-
tal effects such as the greenhouse effect can occur with a strong spatial and temporal offset.
The following production steps are considered during the manufacturing phase:
• Extraction and processing of the raw materials (chemicals)
• Transport to the production sites
• Processing of the lacquer and crosslinker
• Packaging (including packaging material)
• Installation (including transport)
• End-of-life (including transport)
The waste materials and quantities produced are included in the respective modules.
3.3 Estimates and assumptions
If available, datasets which refer to the EU as the geographic reference where chosen (approx. 50%),
otherwise global datasets were used. In cases, where datasets for chemical dispersion where not avail-
able, market for datasets where used, to include transport of the raw materials to the suppliers.
Transport distances for all raw materials used (chemicals, packaging) could be recorded. A payload
factor of 50% was used for all truck transports (suppliers, disposal transports and internal transports),
which corresponds to a full delivery and empty return trip. A data set for a non-specific truck was used.
Page | 6 Dr. Schutz GmbH – PU Color
Dr. Schutz GmbH purchases 100% renewable electricity. 2021 the share of renewable energy sources
on the total renewable energy in Germany was as followed: Wind power: 53.6%; solar power 20.6%;
biomass 18.5%; hydropower 7.3%. Based on this assumption an electricity data set was generated for
the LCA calculation. No CO certificates were considered.
2
For the third-party filler, no data on energy consumption was available, therefore it was assumed, that
the energy consumption for crosslinker production is equally high as for the lacquer. As electricity
source the German electricity mix was taken.
Concerning the waste water during processing, the water is collected and fed back into the process.
According to the manufacturer, almost none processing waste occurs during production. Therefore, a
generic value of 1% production waste was assumed, to cover low amounts of waste. Concerning con-
struction waste, 15% was chosen, which is the recommendation of R<THiNK for product from the cat-
egory “auxiliary and finishing materials”.
Concerning the transport from manufacturer to place of use (A4), an average was calculated based on
the distance of production location to the countries supplied. The installation process was calculated
based on the information material on preparation of floors (compare https://www.dr-schutz.com/wp-
content/uploads/TI_EN_002_Preparation_of_resilient_floorings_200814.pdf; https://www.dr-
schutz.com/wp-content/uploads/PI_EN_PU_Color_200803.pdf). Based on the specific product infor-
mation, two coating processes with 90-100 ml was assumed. As the density of lacquer and crosslinker
are almost 1g/ml, 200 g/m² for total process was taken for calculation.
For installation phase (A5), and module C and D, Germany was chosen as location, as it is the main
market area (compare chapter 2.3).
3.4 Cut-off criteria
All flows which influence is higher than 1% on the total mass, energy or environmental impact are
included in the LCA. It can be assumed that the neglected processes would have contributed less than
5% to the impact categories considered.
All process specific data could be determined and modelled by the use of generic data (EcoInvent 3.6;
EcoInvent 3.8)
3.5 Period under review
The production data have been collected for the year 2021.
3.6 Data quality
For all processes primary data was collected and provided by Dr. Schutz GmbH. The primary data refers
to year 2021. For the data, which is not influenced by the manufacturer, generic data was used. The
secondary data was taken from the database EcoInvent (version 3.6 and 3.8). The database is
maintained on a regular basis and thus meets the requirements of EN 15804 (background data not
older than 10 years). The power sources were chosen from data for Germany in 2021, in accordance
with the geographical and time representativeness. The data quality is very good, because all process
specific data could be documented and modelled by using the generic data.
RETHiNK EPD web application from the company NIBE was used to model the life cycle for the
production and disposal of the declared product systems. To ensure that the results are comparable,
consistent background data from the international database EcoInvent was used in the LCA (e.g. data
records on energy, transport, auxiliary materials, and supplies). Almost all consistent data sets
contained in the EcoInvent database are documented and can be viewed online.
Page | 7 Dr. Schutz GmbH – PU Color
3.7 Allocation
Allocations were avoided as far as possible. There are no coproducts or by-product in the manufactur-
ing of the sealer. Based on energy consumption measurements, the energy demand was allocated to
the individual products. Production waste is collected, recycled and reused internally for other stabili-
sation products.
3.8 Comparability
In principle, a comparison or assessment of the environmental impacts of different products is only
possible if they have been prepared in accordance with EN 15804. For the evaluation of the
comparability, the following aspects have to be considered in particular: PCR used, functional or
declared unit, geographical reference, definition of the system boundary, declared modules, data
selection (primary or secondary data, background database, data quality), scenarios used for use and
disposal phases, and the life cycle inventory (data collection, calculation methods, allocations, validity
period). For further guidance see EN 15804+A2 (5.3 Comparability of EPD for construction products).
Page | 8 Dr. Schutz GmbH – PU Color
4. LCA: Scenarios and additional technical information
According to the preparation guideline (https://www.dr-schutz.com/wp-content/up-
loads/TI_EN_002_Preparation_of_resilient_floorings_200814.pdf), a two-stage cleaning (first with a
cleanser, second only water) is assumed. For the cleanser, a generic dataset from the ecoinvent data-
base is taken (Cleaning consumables, without water, in 13.6% solution state (GLO)| market for), mixed
in the ratio 1:5 and applied with an amount of 200 ml/per m². An overflow or unused portion of 15%
of the prepared sealer is assumed during the installation process.
As the floor covering is disposed as part of the flooring system, the demolition process is not consid-
ered as a load for the calculated system. Therefore, C1 is considered to be zero.
For the production process waste, the EcoInvent scenario Spent solvent mixture {Europe without Swit-
zerland}| treatment of spent solvent mixture, hazardous waste incineration | Cut-off, U was chosen,
which assumes 100% incineration. For the plastic containers and bottles the NMD scenario plastics, via
residue (NMD ID 43) was chosen, which assumes that 80% are incinerated, while 20% are landfilled.
For the sealer itself, 100% incineration was assumed as waste scenario, which fits the waste treatment
of PVC floor covering. The incineration loads were calculated using an EcoInvent dataset for waste
paint.
Note: The transport distances of the waste are based on the standard waste scenarios of the NMD
Determination Method (SBK 2019): incineration 150 km / recycling 50 km / landfill 100 km; vehicle:
truck, unspecific.
For energy recovery, only benefits for plastics were included, as the lower heating value of the chem-
icals was not available. According the EN 15804, loads are credited in A3 or C3 to C4 and benefits are
credited in module D.
For all transports, the environmental profile of a non-specific truck transport was used (conservative
assumption): The vehicle operates with diesel, and it provides a fleet average that includes different
lorry classes as well as EURO classes. This environmental profile contains data for transport, which is
calculated for an average load factor, including empty return trips (EcoInvent 3.6).
5. LCA: Results
The following tables show the results of the impact assessment indicators, resource use, waste and
other output streams. The results presented here refer to the declared specific product.
Disclaimer on ADP-e, ADP-f, WDP, ETP-fw, HTP-c, HTP-nc, SQP: The results of these environmental
impact indicators must be used with caution, as the uncertainties in these results are high or as there
is limited experience with the indicator.
Disclaimer on IRP: This impact category mainly addresses the potential effect of low dose ionizing ra-
diation on human health in the nuclear fuel cycle. It does not consider effects due to possible nuclear
accidents and occupational exposures, nor does it consider radioactive waste disposal in underground
facilities. Potential ionizing radiation from soil, radon, and some building materials is also not measured
by this indicator.
Page | 9 Dr. Schutz GmbH – PU Color
Description of the system boundary
Benefits and loads be-
Construction process
Product stage Use stage End of life stage yond the system bound-
stage
aries
la ir e t a m w a Ry lp p u s t r o p s n a r T g n ir u t c a fu n a M m o r f t r o p s n a r T o t r e r u t c a fu n a me s u fo e c a lp n o it c u r ts n- on C-is s e c o r p n o it a lla ts e s U e c n a n e tn ia M r ia p e R tn e m e c a lp e R tn e m h s ib r u fe R -n e la n o it a r e p Oe s u y g r e -a w la n o it a r e p Oe s u r e t n o it c u r ts n eo Dc -n o itilo m e d / t r o p s n a r T -o r p e ts a Wg n is s e c la s o p s iD y r e v eo s uc ee RR -- ga ni it ln c ye ct o e Rp -l
A1 A2 A3 A4 A5 B1 B2 B3 B4 B5 B6 B7 C1 C2 C3 C4 D
X X X X X MND MND MND MND MND MND MND X X X X X
DE DE DE EU DE - - - - - - - DE DE DE DE DE
X=Module declared | MND=Module not declared
Page | 10 Dr. Schutz GmbH – PU Color
Results of the LCA – Environmental impact: 1 m2 PU Color sealing
Parameter Unit A1 A2 A3 A4 A5 C1 C2 C3 C4 D
Core environmental impact indicators (EN 15804+A2/NMD set 2)
ADP-mm kg Sb-eqv. 8,17E-06 1,75E-07 1,08E-06 4,87E-07 6,19E-06 0,00E+00 9,06E-08 3,29E-08 0,00E+00 -8,38E-08
ADP-f MJ 9,47E+00 1,04E-01 4,00E+00 2,90E-01 4,73E+00 0,00E+00 5,39E-02 3,62E-02 0,00E+00 -6,63E-01
AP mol H+ eqv. 7,22E-03 4,02E-05 6,79E-04 1,11E-04 2,24E-03 0,00E+00 2,07E-05 3,73E-05 0,00E+00 -1,40E-04
EP-fw kg PO4 eqv. 3,00E-05 6,99E-08 6,51E-06 1,94E-07 2,18E-05 0,00E+00 3,61E-08 4,68E-08 0,00E+00 -3,43E-06
EP-m kg N eqv. 7,50E-04 1,42E-05 1,68E-04 3,93E-05 4,19E-04 0,00E+00 7,31E-06 1,66E-05 0,00E+00 -4,14E-05
EP-t mol N eqv. 6,34E-03 1,56E-04 1,49E-03 4,33E-04 3,63E-03 0,00E+00 8,06E-05 1,84E-04 0,00E+00 -3,80E-04
GWP-b kg CO2 eqv. -5,59E-03 3,20E-06 -3,89E-02 8,87E-06 1,61E-02 0,00E+00 1,65E-06 1,72E-05 0,00E+00 3,27E-02
GWP-f kg CO2 eqv. 5,91E-01 6,93E-03 2,56E-01 1,92E-02 4,54E-01 0,00E+00 3,58E-03 4,23E-01 0,00E+00 -4,76E-02
GWP-luluc kg CO2 eqv. 3,31E-04 2,54E-06 2,81E-04 7,04E-06 7,91E-03 0,00E+00 1,31E-06 7,56E-07 0,00E+00 -2,07E-04
GWP-total kg CO2 eqv. 5,86E-01 6,93E-03 2,18E-01 1,92E-02 4,78E-01 0,00E+00 3,58E-03 4,23E-01 0,00E+00 -1,51E-02
ODP kg CFC 11 eqv. 3,19E-06 1,53E-09 5,74E-08 4,24E-09 5,08E-07 0,00E+00 7,89E-10 3,92E-10 0,00E+00 -4,15E-09
POCP kg NMVOC eqv. 2,28E-03 4,46E-05 4,65E-04 1,24E-04 1,03E-03 0,00E+00 2,30E-05 4,53E-05 0,00E+00 -9,01E-05
WDP m3 world eqv. 5,03E-01 3,74E-04 6,52E-02 1,04E-03 2,28E-01 0,00E+00 1,93E-04 -1,75E-03 0,00E+00 -4,28E-03
Additional environmental impact indicators (EN 15804+A2/NMD set 2)
ETP-fw CTUe 3,09E+01 9,32E-02 3,28E+00 2,58E-01 1,10E+01 0,00E+00 4,81E-02 1,14E-01 0,00E+00 -1,33E+00
HTP-c CTUh 1,78E-09 3,02E-12 6,81E-11 8,38E-12 4,89E-10 0,00E+00 1,56E-12 5,42E-10 0,00E+00 -1,42E-11
HTP-nc CTUh 2,83E-08 1,02E-10 7,53E-09 2,83E-10 9,65E-09 0,00E+00 5,26E-11 1,65E-09 0,00E+00 -3,74E-10
IRP kBq U235 eqv. 1,80E-02 4,38E-04 5,21E-03 1,21E-03 1,02E-02 0,00E+00 2,26E-04 7,63E-05 0,00E+00 -1,28E-03
disease
3,80E-08 6,23E-10 5,48E-09 1,73E-09 1,60E-08 0,00E+00 3,22E-10 2,99E-10 0,00E+00 -1,12E-09
PM incidence
SQP 2,78E+00 9,06E-02 1,34E+00 2,51E-01 2,40E+00 0,00E+00 4,68E-02 1,48E-02 0,00E+00 -8,85E-01
ADP-mm=Depletion of abiotic resources-minerals and metals| ADP-f=Depletion of abiotic resources-fossil fuels | AP=Acidification of soil and water | EP-fw =Eutrophication, freshwater | EP-m=Eutrophication marine | EP-
T=Eutrophication, terrestrial | GWP-b=Global warming potential - Biogenic | GWP-f=Global warming potential - Fossil | GWP-luluc=Global warming potential - Land use and land use change |GWP-total=Global warming
potential |ODP=Ozone layer depletion |POCP=Photochemical oxidants creation | WDP=Water use | ETP-fw=Ecotoxicity, freshwater | HTP-c=Human toxicity, cancer | HTP-nc=Human toxicity, non-cancer | IRP=Ionising
radiation, human health | PM=Particulate Matter | SQP=Land use
Page | 11 Dr. Schutz GmbH – PU Color
Results of the LCA – Resource consumption, output streams & waste categories: 1 m2 PU Color sealing
Parameter Unit A1 A2 A3 A4 A5 C1 C2 C3 C4 D
PERE MJ 7,30E-01 1,31E-03 -6,24E-02 3,63E-03 1,54E-01 0,00E+00 6,75E-04 1,02E-03 0,00E+00 1,30E-01
PERM MJ 0,00E+00 0,00E+00 3,76E-01 0,00E+00 5,82E-01 0,00E+00 0,00E+00 0,00E+00 0,00E+00 -3,25E-01
PERT MJ 7,30E-01 1,31E-03 3,14E-01 3,63E-03 7,36E-01 0,00E+00 6,75E-04 1,02E-03 0,00E+00 -1,95E-01
PENRE MJ 1,01E+01 1,11E-01 4,03E+00 3,08E-01 5,03E+00 0,00E+00 5,72E-02 3,92E-02 0,00E+00 -7,21E-01
PENRM MJ 9,22E-02 0,00E+00 2,99E-01 0,00E+00 5,87E-02 0,00E+00 0,00E+00 0,00E+00 0,00E+00 0,00E+00
PENRT MJ 1,02E+01 1,11E-01 4,33E+00 3,08E-01 5,09E+00 0,00E+00 5,72E-02 3,92E-02 0,00E+00 -7,21E-01
SM Kg 0,00E+00 0,00E+00 0,00E+00 0,00E+00 0,00E+00 0,00E+00 0,00E+00 0,00E+00 0,00E+00 0,00E+00
RSF MJ 0,00E+00 0,00E+00 0,00E+00 0,00E+00 0,00E+00 0,00E+00 0,00E+00 0,00E+00 0,00E+00 0,00E+00
NRSF MJ 0,00E+00 0,00E+00 0,00E+00 0,00E+00 0,00E+00 0,00E+00 0,00E+00 0,00E+00 0,00E+00 0,00E+00
FW M3 1,29E-02 1,27E-05 1,69E-03 3,53E-05 6,78E-03 0,00E+00 6,57E-06 3,25E-05 0,00E+00 -2,20E-04
HWD Kg 6,80E-06 2,65E-07 3,07E-06 7,34E-07 4,90E-06 0,00E+00 1,37E-07 5,82E-07 0,00E+00 -6,53E-07
NHWD Kg 2,19E-01 6,63E-03 2,00E-02 1,84E-02 6,78E-02 0,00E+00 3,42E-03 7,06E-03 0,00E+00 -4,55E-03
RWD Kg 1,77E-05 6,86E-07 5,34E-06 1,90E-06 1,11E-05 0,00E+00 3,54E-07 1,01E-07 0,00E+00 -1,53E-06
CRU Kg 0,00E+00 0,00E+00 0,00E+00 0,00E+00 0,00E+00 0,00E+00 0,00E+00 0,00E+00 0,00E+00 0,00E+00
MFR Kg 0,00E+00 0,00E+00 0,00E+00 0,00E+00 2,04E-02 0,00E+00 0,00E+00 0,00E+00 0,00E+00 0,00E+00
MER Kg 0,00E+00 0,00E+00 0,00E+00 0,00E+00 0,00E+00 0,00E+00 0,00E+00 0,00E+00 0,00E+00 0,00E+00
EET MJ 0,00E+00 0,00E+00 0,00E+00 0,00E+00 0,00E+00 0,00E+00 0,00E+00 0,00E+00 0,00E+00 0,00E+00
EEE MJ 0,00E+00 0,00E+00 0,00E+00 0,00E+00 0,00E+00 0,00E+00 0,00E+00 0,00E+00 0,00E+00 0,00E+00
PERE=renewable primary energy ex. raw materials | PERM=renewable primary energy used as raw materials | PERT=renewable primary energy total | PENRE=non-renewable primary energy ex. raw materials | PENRM=non-
renewable primary energy used as raw materials | PENRT=non-renewable primary energy total | SM=use of secondary material | RSF=use of renewable secondary fuels | NRSF=use of non-renewable secondary fuels |
FW=use of net fresh water | HWD=hazardous waste disposed | NHWD=non-hazardous waste disposed | RWD=radioactive waste disposed | CRU=Components for re-use | MFR=Materials for recycling | MER=Materials for
energy recovery | EET=Exported energy thermic| EEE=Exported energy electric
Page | 12 Dr. Schutz GmbH – PU Color
6. LCA: Interpretation
As shown in the figure below, raw material supply (A1) and / or installation process (A5) dominates in
all environmental core indicators. The high influence of the installation phase is due to the use of
cleanser in the preparation of the sealer application, as the amount of cleanser needed is quite high
(200 ml).
In some environmental core indicators the manufacturing phase (A3), has a great impact, which can
be traced back to the gas consumption needed during production. Concerning the Global Warming
Potential, waste processing has a high influence as well, due to the waste treatment process being
incineration.
WDP
POCP
ODP
GWP-total
GWP-luluc
GWP-f
GWP-b
EP-T
EP-m
EP-fw
AP
ADP-f
ADP-mm
-60% -40% -20% 0% 20% 40% 60% 80% 100%
A1 A2 A3 A4 A5 C1 C2 C3 C4 D
Figure 1: Dr. Schutz® PU Color - Impact of the individual modules on the environmental core
indicators
The data quality can be classified as good overall. All relevant process-specific data could be collected
in the operational data collection. Consistent data sets from the EcoInvent database were available for
almost all inputs and outputs. The background data meet the requirements of EN 15804, and the
production data were recorded for the year 2021. The quantities of raw materials and
supplies used as well as energy consumption were recorded for the entire operating year.
Page | 13 Dr. Schutz GmbH – PU Color
7. References
CML-IA April 2013 – Charakterisierungsfaktoren entwickelt durch Institut of Environmental Sciences
(CML): Universität Leiden, Niederlande - http://www.cml.leiden.edu/software/data-cmlia.html
Donndorf, R., Kahle H., Müller, G., Philipp H-J., Taschow, H-J., Wolf, O. (1973): Werkstoffeinsatz und
Korrosionsschutz in der chemischen Industrie. VEB Deutscher Verlag für Grundstoffindustrie Leipzig.
European Commission Joint Research Centre Institute for Prospective Technological Studies (JCR
2014): End-of-waste criteria for waste plastic for conversion, Seville, 2014, doi:10.2791/13033
Klöpffer, W., Grahl B.: Ökobilanz (LCA) – Ein Leitfaden für die Ausbildung und Beruf, Wily-VCH Ver-
lag, Weinheim, 2007
Rosauer, V. (2010): Abschätzung der herstellungsbedingten Qualität und Lebensdauer von Asphalt-
deckschichten mit Hilfe der Risikoanalyse (Estimation of the production-related quality and service
life of asphalt wearing courses with the aid of risk analysis). Technischen Universität Darmstadt, 2010
Stichting Bouwkwaliteit (SBK) – Foundation for Building Quality; “Determination Method: Environmen-
tal Performance of Buildings and Civil Engineering Works”
Stichting Nationale Milieudatabase; Bepalingsmethode Milieuprestatie Bouwwerken; Version 1.0; July
2020; Berekeningswijze voor het bepalen van de milieuprestatie van bouwwerken ge-durende hun
gehele levensduur, gebaseerd op de EN 15804.
Windbranche.de – Das Branchenportal rund um die Windenergie. Wind power and electricity genera-
tion in Great Britain: https://www.windbranche.de/wind/windstrom/windenergie-grossbritannien,
last accessed 19 July 2021.
Standards and laws
ISO 14040:2021-02, Environmental management - Life cycle assessment - Principles and framework
ISO 14044:2020-02, Environmental management - Life cycle assessment - Requirements and guide-
lines
ISO 14025:2011-10: Environmental labels and declarations — Type III environmental declarations —
Principles and procedures EN 13249
EN 15804:2012+A2:2019 Sustainability of construction works — Environmental Product Declarations
— Core rules for the product category of construction products
PCR A: General Program Category Rules for Construction Products from the EPD program Kiwa-Eco-
bility Experts, R.0_2021-07-16
PCR B Resilient, textile and laminate floor coverings - Environmental product declarations – Product
category rules; EN 16810:2017
Page | 14 Dr. Schutz GmbH – PU Color
Publisher Mail DE.Ecobility.Ex-
Kiwa - Ecobility Experts perts@kiwa.com
Kiwa GmbH Web https://www.kiwa.com/de/de
Voltastr.5, 13355 Berlin /uber-kiwa/ecobility-experts/
Germany
Programme operator Mail DE.Ecobility.Ex-
Kiwa - Ecobility Experts perts@kiwa.com
Kiwa GmbH Web https://www.kiwa.com/de/de
Voltastr.5, 13355 Berlin /uber-kiwa/ecobility-experts/
Germany
LCA Practitioner Tel. +49 (0) 30 467761-43
Kiwa GmbH Fax. +49 (0) 30 467761-10
Voltastr.5 Mail DE.Nachhaltigkeit@kiwa.com
13355 Berlin Web https://www.kiwa.com/
Germany
Owner of the declaration Tel. 0228-95352-0
Dr. Schutz GmbH Fax. 0228-95352-29
Holbeinstraße 17 Mail info@dr.schutz.com
53175 Bonn Web www.dr-schutz.com
Germany
Kiwa-Ecobility Experts -
established member of
Page | 15 Dr. Schutz GmbH – PU Color
