ENVIRONMENTAL PRODUCT DECLARATION
as per ISO 14025 and EN 15804+A2
Owner of the Declaration Krinner Schraubfundamente GmbH
Publisher Institut Bauen und Umwelt e.V. (IBU)
Programme holder Institut Bauen und Umwelt e.V. (IBU)
Declaration number EPD-KRI-20230308-IBC1-EN
Issue date 11/09/2023
Valid to 10/09/2028
KRINNER Ground Screws
KRINNER Schraubfundamente
www.ibu-epd.com | https://epd-online.com
1. General Information
KRINNER Schraubfundamente KRINNER Ground Screws
Programme holder Owner of the declaration
IBU – Institut Bauen und Umwelt e.V. Krinner Schraubfundamente GmbH
Hegelplatz 1 Passauer Str. 55
10117 Berlin 94342 Straßkirchen
Germany Germany
Declaration number Declared product / declared unit
EPD­KRI­20230308­IBC1­EN 1 kg ground screws (with the exception of the U­, small G­ and K­series)
manufactured by KRINNER Schraubfundamente GmbH
This declaration is based on the product category rules: Scope:
Structural steels, 01/08/2021 This document is an average EPD for Krinner ground screws (except U­,
(PCR checked and approved by the SVR) small G­ and K­series) manufactured in Germany by KRINNER
Schraubfundamente GmbH. The declared unit refers to the average
production of 1 kg Krinner ground screws. The data collection was carried
Issue date out on a factory­specific basis with current annual data from 2021.
The owner of the Declaration is responsible for the data on which it is
11/09/2023
based and verification thereof.
The owner of the Declaration shall be liable for the underlying information
and evidence; the IBU shall not be liable with respect to manufacturer
Valid to
information, Life Cycle Assessment data, and evidence. This EPD was
10/09/2028 drawn up in accordance with the specifications of the EN 15804+A2. This
standard is referred to as EN 15804 hereinafter.
The owner of the declaration shall be liable for the underlying information
and evidence; the IBU shall not be liable with respect to manufacturer
information, life cycle assessment data and evidences.
The EPD was created according to the specifications of EN 15804+A2. In
the following, the standard will be simplified as EN 15804.
Verification
The standard EN 15804 serves as the core PCR
Independent verification of the declaration and data according to ISO
Dipl.­Ing. Hans Peters
14025:2011
(Chairman of Institut Bauen und Umwelt e.V.)
internally X externally
Florian Pronold Matthias Klingler,
(Managing Director Institut Bauen und Umwelt e.V.) (Independent verifier)
1 Environmental Product Declaration ­ KRINNER Schraubfundamente ­ KRINNER Ground Screws
2. Product
2.1 Product description/Product definition 2.2 Application
Krinner ground screws are tapered steel piles that are inserted KRINNER ground screws are used for buildings and other
into the ground in a rotating manner and can be used to ordinary load­bearing structures according to Eurocode 0, such
transfer axial tensile and compressive forces into the subsoil. as: residential buildings, kindergartens, schools, modular
The ground screws partly replace solid foundations and buildings, halls, tiny houses, garden houses, greenhouses,
basically ensure the load transfer of the structure into the carports, tree houses, holiday homes, hotels, office buildings,
subsoil. For example, the ground screws in the V­series consist workrooms etc., in timber and steel post­and­beam construction
of a 2.0­metre­long base element with a drill point and a top or lightweight steel construction, as well as for noise barriers,
plate as well as any necessary extension elements. The slope protection/securing, staircases, footbridges, containers,
individual sections can be coupled together by means of a plug­ masts, signs, electric charging columns, fencing etc. Ground
in connection and thus extended to the required length. screws can also be used for solid buildings, e.g. as a support
Depending on the type, they have different construction lengths under the floor slab, depending on the required load­bearing
and diameters. The ground screws are driven into the ground to capacity of the project­specific conditions.
the required depth by means of an excavator, for example.
E- Series
The ground screws are made of steel and are hot­dip The ground screws in the E­series are optionally equipped with
galvanised. an eccentric set depending on the application. The eccentric
Krinner ground screws are tapered steel piles that are inserted allows fine adjustment for a perfect, vertical stand of the object
into the ground in a rotating manner and can be used to to be erected. The system is particularly suitable for resonance­
transfer axial tensile and compressive forces into the subsoil. and vibration­resistant mounting of tubular posts and masts, for
The ground screws partly replace solid foundations and example.
basically ensure the load transfer of the structure into the
subsoil. For example, the ground screws in the V­series consist F- Series
of a 2.0­metre­long base element with a drill point and a top The ground screws in the F­series feature round or square
plate as well as any necessary extension elements. The flanges. The resulting fixation of the object to be supported
individual sections can be coupled together by means of a plug­ provides improved stability and safety for large static loads.
in connection and thus extended to the required length.
Depending on the type, they have different construction lengths G- Series
and diameters. The ground screws are driven into the ground to The ground screws in the G­series feature one, three or four
the required depth by means of an excavator, for example. threaded screws. They are therefore particularly suitable for
fast vertical and permanent installation of poles and fence
The ground screws are made of steel and are hot­dip posts, for example.
galvanised.
M-series
The ground screws in the M­series have a centred M­thread,
which enables the object to be supported to be screwed directly
onto the ground screw. This makes it suitable for prefabricated
garages and containers, for example.
U-series
The ground screws in the U­series are specially adapted to the
common dimensions of wooden beams. They are particularly
suitable for easy and fast fastening of horizontal and vertical
timber in carport and wooden terrace construction, for example.
V-series
The ground screws in the V­series are extendable ground
screws. Depending on the project, these ground screws can be
extended and were thus specially developed for projects with
high load­bearing requirements.
X-series
The ground screws in the X­series are customised for special
applications. Depending on the requirements, the foundations
are manufactured to fit precisely and individually.
Fig. 1: All Krinner ground screws are made entirely of steel and
are hot­dip galvanised.
Use of the product is subject to the respective national
specifications at the place of use; in Germany, for example, the
MVV TB and the technical specifications based on these
guidelines.
2 Environmental Product Declaration ­ KRINNER Schraubfundamente ­ KRINNER Ground Screws
automatically.
2.3 Technical Data
The following technical data applies to Krinner ground screws. Corrosion protection
The test standard is EN 1090­2. The finished Krinner ground screws are then hot­dip galvanised
Technical construction data in accordance with ISO 1461 to prevent corrosion during
subsequent use and to maximise the life of the product.
Name Value Unit
Density 7850 kg/m3 Quality management
Modulus of elasticity 212000 N/mm2 Krinner Schraubfundamente GmbH operates in accordance
Coefficient of thermal expansion 11.1 10­6K­1 with an integrated management system to ISO 9001.
Thermal conductivity 54 W/(mK) 2.7 Environment and health during manufacturing
Melting point 1460 °C During the entire manufacturing process, no other health
Electrical conductivity at 20°C 0.15 Ω­1m­1 protection measures are required extending beyond the
standard industrial protection measures for commercial
Minimum yield strength (für Bleche) ­ N/mm2
enterprises.
Minimum tensile strength (für Bleche) ­ N/mm2
Minimum elongation (für Bleche) 26 % The site is certified as follows:
Tensile strength 235 N/mm2 ­ ISO 9001 (Quality Management)
Compressive strength 360 N/mm2
In addition, Krinner Schraubfundamente GmbH supports
Grade of material according to the delivery
10038 ­ ergonomic workplaces and offers all employees annual health
standards
checks. Furthermore, fitness courses are offered throughout the
The products' performance values correspond with the year as well as lunch offers for a balanced diet.
Declaration of Performance in terms of their essential
properties in accordance with DIN EN 1090­2:2018­09, Krinner Schraubfundamente GmbH uses 100% green
Execution of steel structures and aluminium structures – Part 2: electricity.
Technical requirements for steel structures.
2.8 Product processing/Installation
2.4 Delivery status The installation procedure for Krinner ground screws is as
Product size and weight on delivery: follows:
Weight: 0.28 ­ 4.16 kg
Dimensions: 0.04 ­ 0.30 m Measurement of the ground screw position.
Pre­punch a hole that is smaller in diameter than the ground
Accordingly, a declared unit of 1 kg at a dimension of 0.10 m is screw to ensure positioning accuracy.
specified in this EPD. If necessary with harder soil layers: pre­drill.
Screw in the ground screw suitable for load bearing, taking into
2.5 Base materials/Ancillary materials account the installation torque, which is determined in advance
The most important components of Krinner ground screws are: on the basis of experimental investigations.
· Structural steel S235 and S355: 97% If the achieved insertion torque is too low, an extension is
Zinc: 3% attached and the ground screw is screwed into deeper soil
layers until the minimum insertion torque required for the soil is
The product / At least one partial product contains substances reached. The minimum internal torque is defined in advance by
from the ECHA list of candidates of Substances of Very High one or more on­site tests. (V­series only)
Concern (SVHC) (17.06.2022) exceeding 0.1% by mass: no This process can be repeated as often as required until the
ground screw has the necessary insertion resistance. (V­series)
The product / At least one partial product contains other CMR The screwing­in process must be documented for all ground
substances in categories 1A or 1B which are not on the ECHA screws
list, exceeding 0.1% by mass in at least one partial product: no
2.9 Packaging
Biocide products were added to this construction product, or it 50% of Krinner ground screws are loaded in full packaging
has been treated with biocide products (this then concerns a (saran wrap, straps) on wooden pallets/ wooden crates. For the
treated product as defined by the (EU) Regulation on Biocide other 50%, full packaging is dispensed with completely for
Products No. 528/2012): no larger deliveries and the ground screws are only loaded onto
pallets secured with strapping bands in order to avoid
2.6 Manufacture unnecessary packaging waste.
After the steel pipes are delivered, they are cut to length using
saws and lasers. The raw material is ordered so that no waste The preliminary product (steel) is delivered with steel strapping
is produced. If waste does occur due to rejects, it is stored in (tube bundle) and cardboard (welding wire).
containers and collected by a scrap dealer who recycles it A welding coil lies loose on the wooden packaging. This
according to regulations. packaging is recycled.
After assembly, the packaging can be recycled at the
Shaping and further processing construction site.
In several work steps involving cold and hot forming, flame
2.10 Condition of use
cutting and punching, the tubes are thus shaped into their final
conical form, the Krinner tip is formed, and the necessary holes The material composition of Krinner ground screws is not
are made in the profiles. Subsequently, the connection altered during use.
solutions specific to the product are welded to the head side of
the product semi­automatically or by a welding robot. In a final
step, the thread coils are welded onto the profile semi­
3 Environmental Product Declaration ­ KRINNER Schraubfundamente ­ KRINNER Ground Screws
Fire protection
2.11 Environment and health during use
No noteworthy environmental pollution is triggered by Name Value
processing and assembling the products in question. No Building material class A1
special measures need to be taken to protect the environment. Burning droplets s1
According to the present state of knowledge, hazards for air
Smoke gas development d0
and soil cannot arise if the products in question are used
properly and as designated.
Water
Special features of the material composition for the period of No components which are hazardous to water are washed out.
use or environmentally­relevant material­inherent properties This is evident from the Zinc input report.
can be excluded.
Mechanical destruction
Nor does the zinc content of the Krinner ground screws have In the event of mechanical destruction, all substances remain
any negative impact on the environment, as can be seen from bound. There are no relevant impacts on the environment in
the Zinc input report. case of mechanical destruction.
2.12 Reference service life 2.14 Re-use phase
The reference service life could not be determined in Krinner ground screws can be 100% recycled and, after careful
accordance with ISO 15686, as Krinner ground screws are inspection, sent for reuse.
used under a wide variety of conditions.
2.15 Disposal
The waste codes in accordance with the List of Wastes
According to the Corrosion report, the planned service life in
Directive (AVV):
80% of European soils is 100 years.
17 04 05 Iron and steel
2.13 Extraordinary effects
2.16 Further information
Fire
Further information on Krinner Schraubfundamente GmbH
The steel ground screws declared here comply with building
products is available at www.krinner.io.
material class A1 – non­combustible according to EN 13501­1.
3. LCA: Calculation rules
missing details were supplemented by estimates based on
3.1 Declared Unit comparable substitutes or information in the secondary
The Declaration refers to the production of 1 kg of Krinner literature. Any data sets missing in the database were assessed
ground screws as an average product of various ground screw by the author of the LCA.
series manufactured by KRINNER Schraubfundamente GmbH
for the year 2021 (excluding the U­, G­ and K­series). Here, the 3.4 Cut-off criteria
invoiced quantity of the various ground screw sizes related to All relevant data, i.e. all raw materials used in production and
the year under consideration was divided by the total weight of the electric energy used, was taken from an operational data
the products. survey for the LCA. The actual transport distances were applied
or estimated using documented rules for all inputs and outputs
Declared unit
considered. Material and energy flows with a share of < 1%
Name Value Unit
were also considered.
Declared unit 1 kg The sum of ignored processes is less than 5% of the impact
categories. The expenses for providing the infrastructure
3.2 System boundary (machines, buildings etc.) of the entire foreground system were
The LCA considers the system boundaries 'from the cradle to not taken into account. The packaging of the preliminary
the factory gate with Modules C1­C4 and Module D' and follows products and the end product is not considered due to the
the modular structure according to EN 15804. The LCA takes minor mass share (<1%) and relevance for the LCA (GWP [A1­
consideration of the following modules: A3] <1%).
Deconstruction (C1) can be carried out manually using a
A1: Manufacture of preliminary products (e.g. steel tubes, screwing bar or screwing vehicle (deconstruction by vehicle
thread coils, laser parts made of structural steel) and project­ possible within a few minutes (1­3 mins.)), so that both options
specific prefabrication of individual components were ignored here, as the influence was estimated to be very
A2: Transport to manufacturer: Transport of preliminary low (GWP [A­C] <1%).
products to the manufacturing site
3.5 Background data
A3: Manufacturing processes and expenses: Assessment and
project­specific commissioning of the individual components for All background data of relevance for the LCA model was taken
the various versions of the Krinner ground screw series from the ecoinvent 3.8 database. Specific data missing from
C1: Deconstruction of the ground screws upstream processes was taken from the ecoinvent 3.8
C2: Transport to waste treatment database.
C3: Waste management for reuse, recovery and/or recycling
3.6 Data quality
C4: Disposal
Data sets on background data are based on the ecoinvent 3.8
D: Reuse, recovery or recycling potential as net flows and
database. Missing specific data of primary products (e.g. steel
credits or loads
pipes, thread coils etc.) was modelled on the basis of generic
3.3 Estimates and assumptions data sets from ecoinvent 3.8, taking into account country­
All plant­ and process­specific data was made available to the specific conditions. Due to the low vertical range of
author of the LCA by Krinner Schraubfundamente GmbH. Any manufacture, the proportion of primary data in the foreground
4 Environmental Product Declaration ­ KRINNER Schraubfundamente ­ KRINNER Ground Screws
system is low. Krinner ground screws are distributed throughout Allocation for waste
Europe/overseas (worldwide), for which the most generic Due to a lack of data, this study does not consider the product
possible assumptions for recycling were made in the end­of­life packaging for transport to the assembly site, in deviation from
(EoL) phase. A quality assessment was made for technological, the standard requirements for the EPD. Offcuts in production
geographical and temporal representativeness; the overall data (A3) are returned to the process as closed­loop production
quality can be classified as good. waste. The resulting energy gain for avoided environmental
The background data sets used are valid until 2021 without impacts from steel scrap is indicated in Module D. In the end­of­
exception. life scenario, a collection loss of 5% is expected, which is
recorded in the present balance as a landfill process in Module
3.7 Period under review C3. The remaining 95% of the metal is sent for raw material
The volumes of raw materials, energy and waste deployed refer recycling in Module C3. The amount of metal scrap for reuse in
to 2021. It corresponds with the current state of technology and another product system, minus a recycling loss of 5%, is
is therefore representative for the period under review. declared as avoided environmental impact in Module D.
3.8 Geographic Representativeness 3.10 Comparability
Land or region, in which the declared product system is Basically, a comparison or an evaluation of EPD data is only
manufactured, used or handled at the end of the product´s possible if all the data sets to be compared were created
lifespan: Germany according to EN 15804 and the building context, respectively
the product­specific characteristics of performance, are taken
into account. The ecoinvent 3.8 background database was
3.9 Allocation
used. As a general rule, EPD data can only be compared or
Allocation in the foreground system
evaluated when all of the data records to be compared have
The production process does not generate any co­products.
been drawn up in accordance with EN 15804 and the building
The software model applied does not contain any allocations.
context and/or product­specific characteristics are taken into
consideration. The ecoinvent 3.8 background database was
used.
4. LCA: Scenarios and additional technical information
Reference service life
Characteristic product properties of biogenic carbon
The product contains less than 5% biogenic carbon (as a Name ValueUnit
proportion of the total mass of the product), which is why the Reference service life (nach ISO 15686­1, ­2, ­7
100 a
information is omitted in this EPD. The same applies to the und ­8)
packaging materials that fall short of the cut­off criteria in the
present study (cardboard boxes, bubble wrap <1%). End of Life (C1-C4)
Name Value Unit
The following table summarises the results of the LCA. The Steel collected separately 1,00 kg
results of the estimated impact do not make any claims
Steel for recycling (95%) 0,95 kg
regarding impact category limits, exceeding threshold values,
Steel for landfilling (5% recycling loss) 0,05 kg
safety levels or risks. Long­term emissions (> 100 years) are
not taken into consideration in the estimated impact. The
Reuse, recovery and recycling potential (D), relevant
impact assessment is based on the evaluation method in
scenario details
accordance with EN 15804.
Name Value Unit
The reference service life could not be determined according to
ISO 15686. According to the Corrosion report, the design Net steel scrap at the end of the life cycle 0,66 kg
service life in 80% of European soils is 100 years.
This scenario contains a recycling rate of 95%.
5 Environmental Product Declaration ­ KRINNER Schraubfundamente ­ KRINNER Ground Screws
5. LCA: Results
The following table summarises the results of the LCA. The results of the estimated impact do not make any claims regarding impact
category limits, exceeding threshold values, safety levels or risks. Long­term emissions (> 100 years) are not taken into consideration
in the estimated impact. The impact assessment is based on the evaluation method in accordance with EN 15804.
DESCRIPTION OF THE SYSTEM BOUNDARY (X = INCLUDED IN LCA; ND = MODULE OR INDICATOR NOT DECLARED; MNR =
MODULE NOT RELEVANT)
Benefits and
Construction loads beyond
Product stage Use stage End of life stage
process stage the system
boundaries
la ire ta m w a Ry lp p u s tro p s n a rT g n iru tc a fu n a M e h t m o rf tro p s n a rTe tis e h t o t e ta g y lb m e s s A e s U e c n a n e tn ia M ria p e R tn e m e c a lp e R tn e m h s ib ru fe R y g re n e la n o ita re p Oe s u re ta w la n o ita re p Oe s u n o itc u rts n o c ­e Dn o itilo m e d tro p s n a rT g n is s e c o rp e ts a W la s o p s iD ­e s u e R­y re v o c e R­g n ilc y c e Rla itn e to p
A1 A2 A3 A4 A5 B1 B2 B3 B4 B5 B6 B7 C1 C2 C3 C4 D
X X X MND MND MND MND MNR MNR MNR MND MND X X X X X
RESULTS OF THE LCA - ENVIRONMENTAL IMPACT according to EN 15804+A2: 1 kg KRINNER Ground Screws (except U-,
small G- and K-series)
Parameter Unit A1-A3 C1 C2 C3 C4 D
Global Warming Potential total (GWP­total) kg CO 2 eq 2.39E+00 0 5.4E­03 2.4E­03 0 ­1.57E+00
Global Warming Potential fossil fuels (GWP­fossil) kg CO 2 eq 2.38E+00 0 5.4E­03 2.39E­03 0 ­1.57E+00
Global Warming Potential biogenic (GWP­biogenic) kg CO 2 eq 5.07E­03 0 1.9E­06 1.28E­06 0 ­1.93E­03
Global Warming Potential luluc (GWP­luluc) kg CO 2 eq 1.2E­02 0 1.94E­06 7.17E­06 0 ­1.17E­03
Depletion potential of the stratospheric ozone layer (ODP) kg CFC11 eq 1.35E­07 0 1.29E­09 7.81E­10 0 ­7.05E­08
Acidification potential of land and water (AP) mol H+ eq 1.1E­02 0 2.25E­05 1.96E­05 0 ­7.2E­03
Eutrophication potential aquatic freshwater (EP­freshwater) kg P eq 1.12E­03 0 3.36E­07 2.5E­07 0 ­8.07E­04
Eutrophication potential aquatic marine (EP­marine) kg N eq 2.58E­03 0 6.87E­06 6.91E­06 0 ­1.57E­03
Eutrophication potential terrestrial (EP­terrestrial) mol N eq 2.52E­02 0 7.52E­05 7.53E­05 0 ­1.65E­02
Formation potential of tropospheric ozone photochemical oxidants kg NMVOC
1.06E­02 0 2.42E­05 2.18E­05 0 ­7.18E­03
(POCP) eq
Abiotic depletion potential for non fossil resources (ADPE) kg Sb eq 6.95E­05 0 1.24E­08 6.59E­09 0 ­6.27E­05
Abiotic depletion potential for fossil resources (ADPF) MJ 2.61E+01 0 8.42E­02 5.5E­02 0 ­1.6E+01
m3 world eq
Water use (WDP) 9.34E­01 0 2.9E­04 1.93E­03 0 ­4.03E­01
deprived
RESULTS OF THE LCA - INDICATORS TO DESCRIBE RESOURCE USE according to EN 15804+A2: 1 kg KRINNER Ground
Screws (except U-, small G- and K-series)
Parameter Unit A1-A3 C1 C2 C3 C4 D
Renewable primary energy as energy carrier (PERE) MJ 3.28E+00 0 1.07E­03 6.34E­04 0 ­1.6E+00
Renewable primary energy resources as material utilization
MJ 0 0 0 0 0 0
(PERM)
Total use of renewable primary energy resources (PERT) MJ 3.28E+00 0 1.07E­03 6.34E­04 0 ­1.6E+00
Non renewable primary energy as energy carrier (PENRE) MJ 2.77E+01 0 8.94E­02 5.85E­02 0 ­1.7E+01
Non renewable primary energy as material utilization (PENRM) MJ 0 0 0 0 0 0
Total use of non renewable primary energy resources (PENRT) MJ 2.77E+01 0 8.94E­02 5.85E­02 0 ­1.7E+01
Use of secondary material (SM) kg 2.58E­01 0 0 0 0 6.65E­01
Use of renewable secondary fuels (RSF) MJ 0 0 0 0 0 0
Use of non renewable secondary fuels (NRSF) MJ 0 0 0 0 0 0
Use of net fresh water (FW) m3 3.55E­02 0 1E­05 4.67E­05 0 ­1.17E­02
RESULTS OF THE LCA – WASTE CATEGORIES AND OUTPUT FLOWS according to EN 15804+A2:
1 kg KRINNER Ground Screws (except U-, small G- and K-series)
Parameter Unit A1-A3 C1 C2 C3 C4 D
Hazardous waste disposed (HWD) kg 3.84E­04 0 2.04E­07 9.76E­08 0 ­3.41E­04
Non hazardous waste disposed (NHWD) kg 0 0 0 0 0 0
Radioactive waste disposed (RWD) kg 6.3E­05 0 5.7E­07 3.59E­07 0 ­3.04E­05
Components for re­use (CRU) kg 0 0 0 0 0 0
Materials for recycling (MFR) kg 0 0 0 9.03E­01 0 0
Materials for energy recovery (MER) kg 0 0 0 0 0 0
Exported electrical energy (EEE) MJ 0 0 0 0 0 0
Exported thermal energy (EET) MJ 0 0 0 0 0 0
RESULTS OF THE LCA – additional impact categories according to EN 15804+A2-optional:
1 kg KRINNER Ground Screws (except U-, small G- and K-series)
Parameter Unit A1-A3 C1 C2 C3 C4 D
Incidence of disease due to PM emissions (PM) Disease 2.01E­07 0 6.35E­10 3.9E­10 0 ­1.23E­07
6 Environmental Product Declaration ­ KRINNER Schraubfundamente ­ KRINNER Ground Screws
incidence
Human exposure efficiency relative to U235 (IR) kBq U235 eq 1.36E­01 0 4.26E­04 2.49E­04 0 ­6.6E­02
Comparative toxic unit for ecosystems (ETP­fw) CTUe 8.66E+01 0 6.57E­02 3.94E­02 0 ­6.35E+01
Comparative toxic unit for humans (carcinogenic) (HTP­c) CTUh 1.79E­08 0 1.82E­12 1.22E­12 0 ­9.82E­09
Comparative toxic unit for humans (noncarcinogenic) (HTP­nc) CTUh 8.66E­08 0 7.19E­11 3E­11 0 ­4.82E­08
Soil quality index (SQP) SQP 9.89E+00 0 9.68E­02 1.01E­01 0 ­6.04E+00
Disclaimer 1 – for the indicator “Potential Human exposure efficiency relative to U235”. This impact category deals mainly with the
eventual impact of low­dose ionizing radiation on human health of the nuclear fuel cycle. It does not consider effects due to possible
nuclear accidents, occupational exposure or radioactive waste disposal in underground facilities. Potential ionizing radiation from the
soil, radon and from some construction materials is also not measured by this indicator.
Disclaimer 2 – for the indicators “abiotic depletion potential for non­fossil resources”, “abiotic depletion potential for fossil resources”,
“water (user) deprivation potential, deprivation­weighted water consumption”, “potential comparative toxic unit for ecosystems”,
“potential comparative toxic unit for humans – cancerogenic”, “Potential comparative toxic unit for humans ­ not cancerogenic”,
“potential soil quality index”. The results of this environmental impact indicator shall be used with care as the uncertainties on these
results are high as there is limited experience with the indicator.
6. LCA: Interpretation
The following graphic depicts the relative contributions made by
various life cycle processes in the form of a dominance
analysis.
Regardless of the impact category, a similar percentage The eutrophication potential (EP) EP freshwater is 88%, EP salt
distribution of the life cycle phases can be observed with regard water 88% and EP cumulative exceedance 86% determined by
to their impact on total emissions. the preliminary products, followed by manufacturing in A3 with
12% (EP freshwater), 10% (EP salt water) and 1% (EP
The impact categories along the life cycle are predominantly cumulative exceedance).
determined by the supply of raw materials.
The main driver for this is in particular the use of steel and hot­ The photochemical ozone creation potential (POCP) is
dip galvanising, which in total contribute with a share of approx. dominated by the use of raw materials to approx. 91% within
91% to the greenhouse gas potential (GWP) within production manufacturing. Manufacturing in A3 accounts for almost 7%.
(A1­A3).
The consumption of non­fossil abiotic resources (ADP
The product life cycle results in credits (­1.57 kg CO2 equiv.) in elementary) results almost exclusively from the production of
the EoL for subsequent product systems and loads resulting preliminary products (89%) and manufacturing (approx. 9%).
from the net flow calculation for the scrap used in the product.
The consumption of abiotic fossil resources (ADP fossil) within
The ozone depletion potential (ODP) is almost exclusively production (A1­A3) results predominantly from the provision of
determined by the preliminary products (81%). Transport metals (approx. 89%) and processing (approx. 9%). the
contributes 7% and manufacturing 11% to the total emissions provision of metals (approx. 89%) and processing (approx. 9%).
from the manufacturing process.
Within production, the acidification potential (AP) is determined
by the use of primary raw materials and steel (87%).
Galvanising and the energy sources in A3 contribute 12% to the
AP. The share of transport emissions amounts to about 2%.
7 Environmental Product Declaration ­ KRINNER Schraubfundamente ­ KRINNER Ground Screws
7. Requisite evidence
Not of relevance service life in 80% of European soils is 100 years. No product­
specific data is known about empirical values regarding
Krinner ground screws are hot­dip galvanised (corrosion weathering.
protection); according to the Corrosion report, the planned
8. References
Standards
DIN 50929
DIN 50929­1:2017­03, Corrosion of metals – Corrosion ISO 1580
likelihood of metallic materials when subject to corrosion from DIN EN ISO 1580:2011­12, Slotted pan head screws – Product
the outside – Part 1: General grade A (ISO 1580:2011)
EN 12699 Eurocode 0
DIN EN 12699:2015­07, Execution of special geotechnical DIN EN 1990­12, Eurocode 0 – Basis of structural design
works – Displacement piles
Other literature
EN 15804
DIN EN 15804:2022­03, Sustainability of construction works – AVV 2020
Environmental product declarations – Core rules for the Regulation on the European List of Wastes:
construction products product category; German version EN Construction and demolition waste (including excavated soil
15804:2012+A2:2019 + AC:2021 from contaminated sites)
EN 13501-1 BBSR
DIN EN 13501­1:2010­1, Fire classification of construction Federal Institute for Building, Urban Affairs and Regional
products and building elements – Part 1: Classification using Planning (BBSR), Service lives of components. Service lives of
data from reaction to fire tests components for Life Cycle Analyses in accordance with the
evaluation system for sustainable building (BNB), in: German
ISO 14025 Federal Ministry for the Environment, Nature Conservation and
DIN EN ISO 14025: 2011­10, Environmental references and Nuclear Safety (pub.), 2017
declarations – Type III environmental declarations – Principles
and processes German Landfill Directive (DepV), 2009
Directive on landfills and long­term storage (German Landfill
ISO 14040 Directive (DepV), 2009
DIN EN ISO 14040:2021­02, Environmental management – Life
cycle assessment ­ Principles and framework conditions ECHA list
List of approved materials – ECHA – European Union;
ISO 14044 https://echa.europa.eu
DIN EN ISO 14044:2021­02, Environmental management – Life
cycle assessment – Requirements and guidelines ecoinvent 3.8
ecoinvent V 3.8 (2021): eco­inventory database, version 3.8, of
EN 1090-1 the Swiss Centre for Eco­Inventories, Dübendorf;
DIN EN 1090­1:2012­02, Execution of steel structures and www.ecoinvent.ch
aluminium structures – Part 1: Requirements for conformity
assessment of structural components IBU 2022
Institut Bauen und Umwelt e.V. (pub.): Generation of
EN 1090-2 Environmental Product Declarations (EPDs); General principles
DIN EN 1090­2:2018­09, Execution of steel structures and for the EPD range of Institut Bauen und Umwelt e.V. (IBU),
aluminium structures – Part 2: Technical requirements for steel version 2.1, 2022
structures
SimaPro
ISO 9001 Prè Sustainability: SimaPro version 9.4.0.1, 2022
DIN EN ISO 9001: 2015, Quality management systems –
Requirements LCA
K. Walter, B. Grahl: Ökobilanz (LCA). Ein Leitfaden für
ISO 15686 Ausbildung und Beruf (Training and Working Guidelines), Wiley
ISO 15686­1:2011­05, Buildings and constructed assets – 2009
Service life planning – Part 1: General principles and
requirements Ökobaudat 2022
Federal Ministry of Housing, Urban Development and
ISO 1461 Construction – BMWSB (pub.): ÖKOBAUDAT release 2021­II:
DIN EN ISO 1461:2022­08, Hot­dip galvanised coatings on EN 15804+A2 and BNB­conformant data for more than 700
fabricated iron and steel articles – Specifications and test construction products
methods
8 Environmental Product Declaration ­ KRINNER Schraubfundamente ­ KRINNER Ground Screws
PCR, Part A möglichen Zinkeintrages in Boden und Grundwasser aus den
Institut Bauen und Umwelt e.V. (pub.): Product Category Rules Schraubfundamenten beim BV der Solaranlage am Fliegerhorst
for building­related products and services, Part A: Calculation Kaufbeuren (Expert opinion: Determination of a possible zinc
rules for the Life Cycle Assessment and requirements on the input into soil and groundwater from the ground screws at the
project report, in accordance with EN 15804+A2:2019, version BV of the solar plant at the Kaufbeuren air base)
1.3), 31 August 2022
Building regulations of the federal states
PCR: Structural steel Feuer Trutz (2023); State building regulations / Building
Institut Bauen und Umwelt e.V. (pub.): Product Category Rules regulations of the federal states. State building regulations /
for building­related products and services, Part B: Building regulations of the federal states (feuertrutz.de)
Requirements on the EPD for structural steel, version 3, 24 July
2023 MVV TB
Model Administrative Regulation Technical Building Regulations
Corrosion report www.dibt.de/de/wir­bieten/technische­baubestimmungen
Prof.Dr.­Ing.Habil. Prof. H.C. Ulf Nürnberger (expert in
'Corrosion and corrosion protection in the construction KRINNER Schraubfundamente GmbH
industry' (2016): Corrosion protection report on Krinner ground www.krinner.io
screws
Zinc input report
Institute for Soil Mechanics and Foundation Engineering (Univ.
Prof. Dr.­Ing. H. Schulz (2004)): Gutachten Bestimmung eines
9 Environmental Product Declaration ­ KRINNER Schraubfundamente ­ KRINNER Ground Screws
Publisher
Institut Bauen und Umwelt e.V. +49 (0)30 3087748­ 0
Hegelplatz 1 info@ibu­epd.com
10117 Berlin www.ibu­epd.com
Germany
Programme holder
Institut Bauen und Umwelt e.V. +49 (0)30 3087748­ 0
Hegelplatz 1 info@ibu­epd.com
10117 Berlin www.ibu­epd.com
Germany
Author of the Life Cycle Assessment
myclimate Deutschland gGmbH +49 7121 9223 50
Kurrerstr. 40/3 kontakt@myclimate.de
72762 Reutlingen www.myclimate.de
Germany
Owner of the Declaration
Krinner Schraubfundamente GmbH + 49 9424 9401­80
Passauer Str. 55 service@krinner.com
94342 Straßkirchen https://www.krinner.io/
Germany
10 Environmental Product Declaration ­ KRINNER Schraubfundamente ­ KRINNER Ground Screws
