ENVIRONMENTAL PRODUCT DECLARATION
as per ISO 14025 and EN 15804+A2
Owner of the Declaration Hilti Aktiengesellschaft
Publisher Institut Bauen und Umwelt e.V. (IBU)
Programme holder Institut Bauen und Umwelt e.V. (IBU)
Declaration number EPD-HIL-20230388-IBA4-EN
Issue date 12.09.2023
Valid to 30.01.2028
HIT-MM PLUS
Hilti AG
www.ibu-epd.com | https://epd-online.com
1. General Information
Hilti AG HIT-MM PLUS
Programme holder Owner of the declaration
IBU – Institut Bauen und Umwelt e.V. Hilti Aktiengesellschaft
Hegelplatz 1 Feldkircher Strasse 100
10117 Berlin 9494 Schaan
Germany Liechtenstein
Declaration number Declared product / declared unit
EPD-HIL-20230388-IBA4-EN The declared product is a HILTI injectable mortar HIT-MM PLUS. The
declared unit is one kilogram of reaction resin product in the mixing ratio of
the two components necessary for processing. The packaging is also
included in the calculation. The declared unit is stated in [kg].
This declaration is based on the product category rules: Scope:
Reaction resin products, 01.08.2021 This document refers to the injectable mortar HIT-MM PLUS with its
(PCR checked and approved by the SVR) packaging. For the compilation of the life cycle assessment, specific data
were collected from the factory in Kaufering, Germany, of the HILTI AG.
For the compilation of the life cycle assessment, specific data were
Issue date collected from the factory in Kaufering, Germany, of the HILTI AG. Data
from the years 2018 to 2021 are used, which correspond to the annual
12.09.2023
average.
The owner of the declaration shall be liable for the underlying information
and evidence; the IBU shall not be liable with respect to manufacturer
Valid to
information, life cycle assessment data and evidences.
30.01.2028
The EPD was created according to the specifications of EN 15804+A2. In
the following, the standard will be simplified as EN 15804.
Verification
The standard EN 15804 serves as the core PCR
Independent verification of the declaration and data according to ISO
14025:2011
internally X externally
Dipl.-Ing. Hans Peters
(Chairman of Institut Bauen und Umwelt e.V.)
Florian Pronold Matthias Klingler,
(Managing Director Institut Bauen und Umwelt e.V.) (Independent verifier)
1 Environmental Product Declaration - Hilti AG - HIT-MM PLUS
2. Product
2.1 Product description/Product definition ETA 16/0239
The declared product of HIT-MM PLUS is a two-component ETA 17/0199
system. The resin component (component A) comprises a resin
based on methacrylate as well as mineral and cementitious Shelf life:
fillers. The curing agent component (component B) comprises 12 months
peroxide hardener, water and mineral fillers. Mixing the two
components A and B in the static mixer initiates the curing Substrate temperature during installation:
(hardening) reaction of both binder systems. During the curing +5°C to +25 °C
phase, a very strong bond is formed between the organic and
inorganic binder matrix. The hybrid system formed during Working time:
cement and resin curing results in a crosslinked duromer with > 0°C to 5 °C 10 min
desired design properties (high bond strengths within a short > 5°C to +10 °C 8 min
curing time) and particular durability. Composite foils are used > 10°C to +20 °C 5 min
for the two-component foil pack of HIT-MM PLUS. This kind of > 20°C to +30 °C 3 min
packaging serves the following purposes: waste volume > 30°C to +40 °C 2 min
reduction, easy storage and transport, and less packaging
material. Curing time:
> 0°C to 5 °C 2.5 hours
Through legislation and increased public awareness users have > 5°C to +10 °C 1.5 hours
increasingly become discerned towards the use of styrene and > 10°C to +20 °C 45 min
other highly volatile components with their resulting unpleasant > 20°C to +30 °C 30 min
odour and low flash point (flammability). > 30°C to +40 °C 20 min
The reaction resins used in all Hilti hybrid adhesives contain no 2.4 Delivery status
styrene, are practically odourless and have a considerably The product Hilti HIT-MM PLUS is available in foil-packages
higher flash point, i.e. higher than 100 °C in comparison to 34 with a total of 330 ml and 500 ml injectable mortar in the
°C for styrene based products. HIT-MM PLUS is a premium corresponding mixing ratio.
performance injectable hybrid mortar with approvals for rebar
connections and heavy-duty anchoring. For the placing of the 2.5 Base materials/Ancillary materials
product on the market in the European Union European Free Hilti HIT-MM PLUS is supplied in the form of a dual component
Trade Association EU/EFTA) (with the exception of Switzerland) film-wrapped pack comprising a resin component and a curing
the Regulation (EU) No. 305/2011 (CPR) applies. The product agent component at a volume ratio of 3:1. The mixing ratio of
needs a declaration of performance taking into consideration resin and curing agent components is automatically set during
the following European Technical Approvals the injection process. Product curing commences directly after
the components are mixed.
ETA 16/0239
ETA 17/0199 The product reviewed in this EPD contains the following
component volumes:
and the CE marking. For the application and use the respective
national provisions apply. Resin component:
Methacrylate resin mixture: 40 to 50 % by weight
2.2 Application Mineral fillers: 30 to 40 % by weight
Hilti HIT-MM PLUS serves for safely securing threaded rods Cement: 10 to 20 % by weight
and post-installed rebar connections in uncracked concrete Other: < 5 % by weight
C20/25 to concrete ≥ C20/25 (B25).
During installation the use of Hilti HDE22 dispenser with the Curing agent component:
Volume Calculator App leads to no under or over fill, reducing Mineral fillers: 50 to 60 % by weight
underfilling related risks and minimizing mortar wastage. Water: 20 to 30 % by weight
Dibenzoyl peroxide: 5 to 10 % by weight
2.3 Technical Data Other: < 6 % by weight
Constructional data
This product article contains substances listed in the candidate
Name Value Unit
list (date: 30.06.2022) exceeding 0.1 percentage by mass: no.
Density acc. to ISO 2811-1 1710 kg/m3
Compressive strength (20°C) acc. to EN ISO 604 79 N/mm2 This product contains other Carcinogenic, Mutagenic,
Elastic modulus (pressure) acc. to EN ISO 604 2096 N/mm2 Reprotoxic (CMR) substances in categories 1A or 1B which are
not on the candidate list, exceeding 0.1 percentage by mass:
Tensile strength (20°C) acc. to EN ISO 527-1;
14,4 N/mm2 no.
type 1A - EN ISO 527-2
Tensile modulus acc. to EN ISO 527-1; type 1A - 3697 N/mm2 Biocide products were added to this construction product or it
EN ISO 527-2 has been treated with biocide products (this then concerns a
Hilti HIT-MM PLUS displays the following characteristics: treated product as defined by the (EU) Ordinance on Biocide
Products No. 528/2012): no.
Performance data of the product in accordance with the
2.6 Manufacture
declaration of performance with respect to its essential
characteristics according to
2 Environmental Product Declaration - Hilti AG - HIT-MM PLUS
Most raw materials are sourced in Europe. The transport is of the product should be between +5 °C to +25 °C during
exclusively by truck for the European raw materials, and by storage and +5°C to +40°C during usage. Hilti literature and
truck and by ship for the others. Chemical mortars are usually official approvals must always be considered. The two
two-component systems consisting of a binder and a hardener. components of HIT-MM PLUS are only for use in combination
One of the base components of the binder is the reactive resin with the defined volume ratio and under the conditions
which in the case of HIT-MM PLUS is produced in Kaufering. mentioned above to build up a crosslinked filled duromer.
The resin production process is a chemical reaction of the
corresponding educts to a basic resin with subsequent mixing 2.11 Environment and health during use
of the basic resin with different reactive diluents to a reactive Refer to the Safety Data Sheet (SDS) for detailed information
resin. This process is controlled and monitored by process on handling, storage as well as first aid, firefighting and
control technology. The production of chemical mortars consists accidental release measures and disposal considerations.
of a mixing process and a filling process of the respective single Following the given instructions help to minimize the risk to
components (binder and hardener) and their subsequent union health and environment.
to a two-component system (packaging). Here as well process
2.12 Reference service life
control technology is used to weigh and mix solid and liquid
compounds according to the specification. In the next step both Hilti HIT-MM PLUS is exposed to a wide variety of
well-mixed components run through an automized filling line in environmental factors during the use phase. The anticipated
which each of the processed masses is filled into a tubular foil Reference Service Life depends on the specific installation
bag. Finally the single components are combined in one situation and the product exposure scenario. The main factors
packaging unit. The two-pack foil bags are packed into influencing the period of use involve weathering as well as
cardboard boxes and then finally shipped. The manufacturing mechanical loads and chemical exposure.
plant of HIT-MM PLUS, Hilti GmbH Industriegesellschaft für Description of the influences on the ageing of the product when
Befestigungstechnik, Hiltistr. 6, 86916 Kaufering, Germany, is applied in accordance with the rules of technology.
certified according to ISO 9001. The guideline defines
international standards for quality and process management.
2.13 Extraordinary effects
2.7 Environment and health during manufacturing Fire
Even without any special fire safety features the Injection
The manufacturing plant of HIT-MM PLUS,Hilti GmbH
Systems comply with at least the requirements of the DIN EN
Industriegesellschaft für Befestigungstechnik, Hiltistr. 6, 86916
13501-1 standard for fire classes E and Efl. As crosslinked
Kaufering, Germany, is certified according to ISO 14001 which
methacrylate resins do not melt or drip, the resins do not
defines international standards for sustainable environmental
contribute towards spreading fire. Apart from the common
management. The production site is also certified in
combustion produces carbon monoxide and carbon dioxide, fire
accordance with ISO 50001 Energy Management Systems.
gases can contain traces of methyl methacrylate, esters,
2.8 Product processing/Installation alcohol, and hydrocarbons. Due to the quantities used, they
The product is delivered with Instructions for Use explaining the only have a subordinate influence on the fire characteristics of
basic steps for installation: a building structure in which they have been installed.
1) For safe handling the precautionary measures described in Fire protection
the Safety Data Sheet (SDS) (e.g. hand and eye protection)
Name Value
must be adhered to
Building material class E/Efl
2) Insert the cartridge into the black cassette
3) Screw on the mixing nozzle Burning droplets No performance assessed
4) Put the cassette into the dispenser system Smoke gas development No performance assessed
5) Discard the first trigger pulls
6) Fill 2/3 of the borehole with mortar
Water
7) Set the fixing element
The cured product is chemically inert and insoluble in water.
HIT-MM PLUS is certified for use as an anchoring adhesive in
After mixing the components and squeezing the mortar into the
concrete for water treatment applications according to National
borehole the fixing element has to be set within the working
Sanitation Foundation (US) NSF.
time mentioned in the Instructions for Use. After the curing time,
described as well in the Instructions for Use, the mortar is ready
Mechanical destruction
to take up loads.
It is recommended to use dust protection during the demolition
2.9 Packaging of the cured chemical anchor.
Hilti HIT-MM PLUS is supplied in the form of a 2-foil-pack
2.14 Re-use phase
system and thus leads to very little waste remaining after use
The product cannot be reused. After usage the product can be
on the construction site. After curing, the product can be
removed by demolition.
disposed of with household waste. Full or only partially emptied
cartridges must be disposed of as special waste in accordance 2.15 Disposal
with official regulations. The outer packaging consisting of
Uncured Hilti HIT-MM PLUS can be disposed of according to
plastic foil and cardboard boxes designed according to the
the European waste code 08 04 09* or 20 01 27*. The built-in
product size can be recycled. Packaging contaminated by the
cured anchor can be disposed as construction waste for which
product must be disposed in a safe manner in accordance with
the European waste code 17 01 01 applies.
local/national regulations.
2.16 Further information
2.10 Condition of use
Further information is available on request under
During the installation the temperature of the base material
anchor.hse@hilti.com and on the Hilti website: www.hilti.group
must be between 0 °C and 40 °C during application - Exception
in solid clay brick: between +5 °C and 40 °C. The temperature
3 Environmental Product Declaration - Hilti AG - HIT-MM PLUS
3. LCA: Calculation rules
3.1 Declared Unit
The product declared here is an injection mortar from HILTI AG
with the designation HIT-MM PLUS. The declared unit refers to
1 kg reaction resin product in the mixing ratio of the two
components required for processing. The packaging, based on
1 kg of reaction resin product, is also calculated at 0.149 kg.
The table below shows the data of the declared unit.
Declared unit
Name Value Unit
Declared unit 1 kg
3.2 System boundary
Type of EPD:
cradle to gate with options.The following information modules
are defined as system boundaries in this study:
Illustration 2: Information module A1 to A3 of product (part
2)
Production stage (A1- A3):
• A1, raw material extraction,
• A2, transport to manufacturer,
• A3, manufacture.
End of life (C1- C4):
• C1, dismantling/demolition,
• C2, transportation,
• C3, waste treatment,
• C4, elimination.
Reuse, recovery and recycling potential (D)
In order to precisely record the indicators and environmental
impacts of the declared unit, a total of 8 information modules
are considered. The information modules A1 to A3 describe the
provision of materials, the transport to the production site and
the production processes of the product itself.
The main products are sourced from the European Union and
Asia. Transport is by truck and ship. The following flow charts Illustration 3: Information module A1 to A3 of packaging
illustrate the underlying production process.
3.3 Estimates and assumptions
The electricity mixes and other background data are calculated
on a country-specific basis for the production processes. For
1,1'-(p-tolylimino)dipropan-2-ol and 1,2-dihydroxybenzene, an
assumption was made for the calculation of the material supply.
This assumption is based on manufacturer data. No
assumptions or limitations were made for other formulation
contents or processes.
3.4 Cut-off criteria
All energy and mass inputs were taken into account.The cut-off
criterion according to EN 15804 is not applied.
3.5 Background data
The database of the background data of the GaBi 10 and
ecoinvent 3.8 databases, to which this study also refers, is
documented under the following link. (Sphera).
3.6 Data quality
For the compilation of the life cycle assessment, specific data
were collected from the factory Kaufering, in Germany, of the
Illustration 1: Information module A1 to A3 of product (part HILTI AG from the year 2022. The background data from the
1) /GaBi 10 database/ used is from the year 2022 and thus of high
relevance. The mass of the different components of the reactive
resin mixture come from the information to the recipe. The data
quality is classified as appropriate.
3.7 Period under review
4 Environmental Product Declaration - Hilti AG - HIT-MM PLUS
Data from 2022 is used as production has only just started. energy credits resulting therefrom are completely charged in
modules A1-A3.
3.8 Geographic Representativeness No further allocations are made.
Land or region, in which the declared product system is
manufactured, used or handled at the end of the product´s 3.10 Comparability
lifespan: Germany Basically, a comparison or an evaluation of EPD data is only
possible if all the data sets to be compared were created
according to EN 15804 and the building context, respectively
3.9 Allocation
the product-specific characteristics of performance, are taken
Allocation of co-products takes place in the information into account.
modules A1-A3. The production waste of the injection-moulded
components is thermally recovered. The electrical and thermal
4. LCA: Scenarios and additional technical information
End of life (C1-C4)
Characteristic product properties of biogenic carbon
The product is demolished using an electric chisel. The
No renewable raw materials are used in the product. Therefore,
electrical energy consumption for the tool is assumed to be
the biogenic carbon is shown as zero. The following raw
0.05 MJ for the declared unit. The electricity consumption is
materials contain biogenic carbon in the packaging.
calculated with a European electricity mix. The construction
Information on describing the biogenic Carbon Content at waste is transported by truck 50 km to the waste treatment
factory gate plant.
Name Value Unit The construction waste is shredded in the waste treatment
Packaging Cardboard Box 0,013 kg C plant and then dumped.
Packaging IfU-Lables, Paper 0,014 kg C Name Value Unit
Collected as mixed construction waste 1 kg
Crushing in the shredder 1 kg
Landfilling 1 kg
Information on packaging
Name Value Unit Reuse, recovery and/or recycling potentials (D), relevant
Componsite foil PE/PET (foil bags) 0,0089 kg scenario information
Clips, Aluminium 0,0030 kg In this calculation there are no reuse, recovery and recycling
Connector, PBT 0,0204 kg potentials. Therefore, the information module D is declared and
shown as zero.
Composite foil, PE-LD 0,0092 kg
Name Value Unit
Mixer, PP 0,0390 kg
Reuse, recovery and recycling potentials 0 kg
Mixer extension, PE-LD 0,0050 kg
IfU- Labels, Paper 0,0333 kg
Cardboard box 0,0301 kg
5 Environmental Product Declaration - Hilti AG - HIT-MM PLUS
5. LCA: Results
DESCRIPTION OF THE SYSTEM BOUNDARY (X = INCLUDED IN LCA; ND = MODULE OR INDICATOR NOT DECLARED; MNR =
MODULE NOT RELEVANT)
Benefits and
Construction loads beyond
Product stage Use stage End of life stage
process stage the system
boundaries
la ire ta m w a Ry lp p u s tro p s n a rT g n iru tc a fu n a M e h t m o rf tro p s n a rTe tis e h t o t e ta g y lb m e s s A e s U e c n a n e tn ia M ria p e R tn e m e c a lp e R tn e m h s ib ru fe R y g re n e la n o ita re p Oe s u re ta w la n o ita re p Oe s u n o itc u rts n o c -e Dn o itilo m e d tro p s n a rT g n is s e c o rp e ts a W la s o p s iD -e s u e R-y re v o c e R-g n ilc y c e Rla itn e to p
A1 A2 A3 A4 A5 B1 B2 B3 B4 B5 B6 B7 C1 C2 C3 C4 D
X X X MND MND MND MND MNR MNR MNR MND MND X X X X X
RESULTS OF THE LCA - ENVIRONMENTAL IMPACT according to EN 15804+A2: 1 kg HIT-MM PLUS
Parameter Unit A1-A3 C1 C2 C3 C4 D
Global Warming Potential total (GWP-total) kg CO 2 eq 2.32E+00 5.12E-03 3.76E-03 2.6E-03 1.45E-02 0
Global Warming Potential fossil fuels (GWP-fossil) kg CO 2 eq 2.32E+00 5.12E-03 3.74E-03 2.59E-03 1.45E-02 0
Global Warming Potential biogenic (GWP-biogenic) kg CO 2 eq 0 0 0 0 0 0
Global Warming Potential luluc (GWP-luluc) kg CO 2 eq 9.14E-04 1.08E-06 2.07E-05 1.2E-05 2.67E-05 0
Depletion potential of the stratospheric ozone layer (ODP) kg CFC11 eq 2.19E-08 7.5E-14 2.22E-16 3.85E-15 3.4E-14 0
Acidification potential of land and water (AP) mol H+ eq 5.42E-03 1.12E-05 1.17E-05 1.34E-05 1.03E-04 0
Eutrophication potential aquatic freshwater (EP-freshwater) kg P eq 7.94E-05 1.49E-08 1.11E-08 7.43E-09 2.45E-08 0
Eutrophication potential aquatic marine (EP-marine) kg N eq 1.46E-03 2.52E-06 5.37E-06 6.11E-06 2.62E-05 0
Eutrophication potential terrestrial (EP-terrestrial) mol N eq 1.57E-02 2.65E-05 6.01E-05 6.74E-05 2.88E-04 0
Formation potential of tropospheric ozone photochemical oxidants kg NMVOC
4.37E-03 6.82E-06 1.05E-05 1.66E-05 7.97E-05 0
(POCP) eq
Abiotic depletion potential for non fossil resources (ADPE) kg Sb eq 4.07E-06 1.4E-09 3.1E-10 2.87E-09 1.48E-09 0
Abiotic depletion potential for fossil resources (ADPF) MJ 4.72E+01 9.29E-02 4.96E-02 5.06E-02 1.9E-01 0
m3 world eq
Water use (WDP) 2.14E-01 1.17E-03 3.33E-05 4.99E-04 1.59E-03 0
deprived
RESULTS OF THE LCA - INDICATORS TO DESCRIBE RESOURCE USE according to EN 15804+A2: 1 kg HIT-MM PLUS
Parameter Unit A1-A3 C1 C2 C3 C4 D
Renewable primary energy as energy carrier (PERE) MJ 5.86E+00 5.16E-02 2.82E-03 4.06E-03 2.85E-02 0
Renewable primary energy resources as material utilization
MJ 9.5E-01 0 0 0 0 0
(PERM)
Total use of renewable primary energy resources (PERT) MJ 6.81E+00 5.16E-02 2.82E-03 4.06E-03 2.85E-02 0
Non renewable primary energy as energy carrier (PENRE) MJ 4.37E+01 9.3E-02 4.97E-02 5.07E-02 1.9E-01 0
Non renewable primary energy as material utilization (PENRM) MJ 3.59E+00 0 0 0 0 0
Total use of non renewable primary energy resources (PENRT) MJ 4.73E+01 9.3E-02 4.97E-02 5.07E-02 1.9E-01 0
Use of secondary material (SM) kg 6.97E-02 0 0 0 0 0
Use of renewable secondary fuels (RSF) MJ 0 0 0 0 0 0
Use of non renewable secondary fuels (NRSF) MJ 0 0 0 0 0 0
Use of net fresh water (FW) m3 9.71E-03 4.92E-05 3.19E-06 1.42E-05 4.82E-05 0
RESULTS OF THE LCA – WASTE CATEGORIES AND OUTPUT FLOWS according to EN 15804+A2:
1 kg HIT-MM PLUS
Parameter Unit A1-A3 C1 C2 C3 C4 D
Hazardous waste disposed (HWD) kg 2.38E-08 8.04E-12 2.38E-13 6.34E-13 9.75E-12 0
Non hazardous waste disposed (NHWD) kg 5.03E-02 7E-05 7.13E-06 1.34E-05 9.71E-01 0
Radioactive waste disposed (RWD) kg 7.24E-04 1.49E-05 6.13E-08 6.68E-07 2.11E-06 0
Components for re-use (CRU) kg 0 0 0 0 0 0
Materials for recycling (MFR) kg 0 0 0 0 0 0
Materials for energy recovery (MER) kg 0 0 0 0 0 0
Exported electrical energy (EEE) MJ 0 0 0 0 0 0
Exported thermal energy (EET) MJ 0 0 0 0 0 0
RESULTS OF THE LCA – additional impact categories according to EN 15804+A2-optional:
1 kg HIT-MM PLUS
Parameter Unit A1-A3 C1 C2 C3 C4 D
Disease
Incidence of disease due to PM emissions (PM) ND ND ND ND ND ND
incidence
Human exposure efficiency relative to U235 (IR) kBq U235 eq ND ND ND ND ND ND
Comparative toxic unit for ecosystems (ETP-fw) CTUe ND ND ND ND ND ND
Comparative toxic unit for humans (carcinogenic) (HTP-c) CTUh ND ND ND ND ND ND
Comparative toxic unit for humans (noncarcinogenic) (HTP-nc) CTUh ND ND ND ND ND ND
6 Environmental Product Declaration - Hilti AG - HIT-MM PLUS
Soil quality index (SQP) SQP ND ND ND ND ND ND
The secondary material (SM) used leads from paper production.
Disclaimer 2 – for the indicators 'abiotic depletion potential for non-fossil resources', 'abiotic depletion potential for fossil resources',
'water (user) deprivation potential, deprivation-weighted water consumption', 'potential comparative toxic unit for ecosystems', 'potential
comparative toxic unit for humans – cancerogenic', 'Potential comparative toxic unit for humans - not cancerogenic', 'potential soil
quality index'. The results of this environmental impact indicator shall be used with care as the uncertainties on these results are high
as there is limited experience with the indicator.
6. LCA: Interpretation
The dominance analysis shows that the main causes for the Illustration: Dominance analysis A1
environmental impacts and indicators can be found in
information module A1. This shows the total global warming Within the reaction resin mixture itself, about 40% of the
potential for material provision at around 92%, based on all total global warming potential and about 39% of the total
information modules. With the total non-renewable primary non-renewable primary energy are created by the material
energy it is about 95%. provision of the UMA 201. The HPMA has a share of
approx. 28% of the total greenhouse gas emissions and
approx. 30% of the total non-renewable primary energy.
Illustration: Dominance analysis A1- A3
If you look at the material provision of the reaction resin
mixture and the packaging in detail, it becomes clear which
raw materials make a decisive contribution to the Illustration: Dominance analysis A1, reaction resin mixture
respective environmental effects and indicators.
The reaction resin mixture itself accounts for 87% of the
total global warming potential in information module A1.
Approx. 5% is accounted for by the PBT of the connector
and approx. 3% by the PP of the mixer.
7. Requisite evidence
Hilti HIT-MM PLUS complies with the requirements of
AgBB overview of results (28 days [µg/m³])
• DIBt (2010) in combination with the NIK values from Name Value Unit
AgBB (2021) for applications in interior areas,
TVOC (C6 - C16) <1000 μg/m3
• emission class A+ outlined in the French VOC Directives
(2019) in accordance with the Eurofins attestation, Sum SVOC (C16 - C22) <100 μg/m3
• CDPH/EHLB Standard Method V 1.2 (2017) in R (dimensionless) <1 -
accordance with Eurofins test report, No. 392-2022- VOC without NIK <100 μg/m3
00035301_C_EN, Eurofins test report, No. 392-2022-
Carcinogenic Substances <1 μg/m3
00035301_E_EN and Eurofins test report, No. 392-
2022-00035302_H_EN respectively.
8. References
7 Environmental Product Declaration - Hilti AG - HIT-MM PLUS
EN ISO 604
EN ISO 604: 2003-12, Kunststoffe - Bestimmung von ecoinvent 3.8
Druckeigenschaften Backgroun data: ecoinvent 3.8
Zürich: ecoinvent
EN 13501-1 http://www.ecoinvent.org
EN 13501-1: 2019-05, Klassifizierung von Bauprodukten und (28.09.2022)
Bauarten zu ihrem Brandverhalten - Teil 1: Klassifizierung mit
den Ergebnissen aus den Prüfungen zum Brandverhalten von ETA 16/0239
Bauprodukten European Technical Approval Hilti HIT-MM PLUS
EN 15804 ETA 17/0199
EN 15804+A2:2019+AC:2021, Sustainability of construction European Technical Approval Hilti HIT-MM PLUS
works — Environmental Product Declarations — Core rules for
the product category of construction products Eurofins test report, No. 392-2022-00035301_C_EN
VOC test report for verification of compliance with
ISO 14001 DIBt(2010)/AgBB(2021)
ISO 14001: 2015-09, Umweltmanagementsysteme -
Anforderungen mit Anleitung zur Anwendung Eurofins test report, No. 392-2022-00035301_E_EN
VOC test report for verification of compliance with the French
ISO 14025 directive from 2010
DIN EN /ISO 14025:2011-10/, Environmental labels and
declarations — Type III environmental declarations — Eurofins test report, No. 392-2022-00035302_H_EN
Principles and procedures VOC test report for verification of compliance with
CDPH/EHLB/Standard Method V1.2 from 2017
ISO 2811-1
ISO 2811-1: 2016-08, Beschichtungsstoffe - Bestimmung der European Waste code
Dichte - Teil 1: Pyknometer-Verfahren in accordance with the European Waste Catalogue (EWC)
(EWC 2014/955/EU) Commission Decision amending Decision
ISO 50001 2000/532/EC on the list of waste pursuant to Directive
ISO 50001: 2018-08, Energiemanagementsysteme - 2008/98/EC of the European Parliament and of the Council
Anforderungen mit Anleitung zur Anwendung
French VOC Directives
ISO 527-1 Décret no 2011321 du 23 mars 2011 relatif à l'étiquetage des
ISO 527-1: 2019-07, Kunststoffe - Bestimmung der produits de construction ou de revêtement de mur ou de sol et
Zugeigenschaften - Teil 1: Allgemeine Grundsätze des peintures et vernis sur leurs émissions de polluants volatils
Arrêté du 19 avril 2011 relatif à l'étiquetage des produits de
ISO 9001 construction ou de revêtement de mur ou de sol et des
ISO 9001: 2015-11, Qualitätsmanagementsysteme - peintures et vernis sur leurs émissions de polluants volatils
Anforderungen
IBU 2021
AgBB (2021) General Instructions for the EPD programme of Institut Bauen
Vorgehensweise bei der gesundheitlichen Bewertung der und Umwelt e.V. Version 2.0,
Emissionen von flüchtigen organischen Verbindungen (VVOC, Berlin: Institut Bauen und Umwelt e.V.,2021
VOC und SVOC) aus Bauprodukten (2021) www.ibu-epd.de
Candidate List of substances of very high concern for Product category rules for construction products – Part B
Authorisation Reaction resin products, 01.2019
European Cheminals Agency (ECHA), in accordance with
Article 50(10) of the REACH regulation Regulation (EU) No. 305/2011 (CPR)
Regulation (EU) No 305/2011 of the European Parliament and
CDPH/EHLB/Standard Method V1.2 of the Council of 9 March 2011 laying down harmonised
California CDPH Standard Method is a US standard for conditions for the marketing of construction products and
evaluating and restricting VOC emissions to indoor air. repealing Council Directive 89/106/EEC Text with EEA
Developed in California as "Section 01350" Specification, relevance
several systems in the US refer to CDPH Standard Method
Sphera
Calculation rules: PCR - Part A GaBi 10 Software: Ganzheitliche Bilanzierung, Leinfelden-
Institut Bauen und Umwelt e.V. (IBU), 2022. Product Category Echterdingen; Sphera Solution GmbH,
Rules for Building-Related Products and Services. Part A: https://gabi.sphera.com/databases/gabi-data-search/
Calculation rules for the life cycle assessment and (28.09.2022)
requirements on the project report. Version 1.3 (08.2022) The literature referred to in the Environmental Product
Declaration must be listed in full.Standards already fully quoted
DIBt (2010) in the EPD do not need to be listed here again.
Grundsätze zur gesundheitlichen Bewertung von Bauprodukten The current version of PCR Part A and PCR Part B of the PCR
in Innenräumen (Oktober 2010) document on which they are based must be referenced.
8 Environmental Product Declaration - Hilti AG - HIT-MM PLUS
Publisher
Institut Bauen und Umwelt e.V. +49 (0)30 3087748- 0
Hegelplatz 1 info@ibu-epd.com
10117 Berlin www.ibu-epd.com
Germany
Programme holder
Institut Bauen und Umwelt e.V. +49 (0)30 3087748- 0
Hegelplatz 1 info@ibu-epd.com
10117 Berlin www.ibu-epd.com
Germany
Author of the Life Cycle Assessment
FIT-Umwelttechnik GmbH 05362 72 69 474
Westerstr. 13 bertram@fit-umwelttechnik.de
38442 Wolfsburg www.fit-umwelttechnik.com
Germany
Owner of the Declaration
Hilti Aktiengesellschaft +423 234 2111
Feldkircher Strasse 100 HAGHSE@hilti.com
9494 Schaan www.hilti.com
Liechtenstein
9 Environmental Product Declaration - Hilti AG - HIT-MM PLUS
