ENVIRONMENTAL PRODUCT DECLARATION
as per ISO 14025 and EN 15804+A2
Owner of the Declaration Grundfos Holding A/S
Publisher Institut Bauen und Umwelt e.V. (IBU)
Programme holder Institut Bauen und Umwelt e.V. (IBU)
Declaration number EPD-GRU-20240274-CBA1-EN
Issue date 01/08/2024
Valid to 31/07/2029
MAGNA3 25,32-40/60/80/100/120, 32-40/60/80/100 F, 40-40/60 F
(Stainless steel)
Grundfos Holding A/S
www.ibu-epd.com | https://epd-online.com
General Information
Grundfos Holding A/S MAGNA3 25,32-40/60/80/100/120, 32-40/60/80/100 F,
40-40/60 F (Stainless steel)
Programme holder Owner of the declaration
IBU – Institut Bauen und Umwelt e.V. Grundfos Holding A/S
Hegelplatz 1 Poul Due Jensens Vej 7
10117 Berlin 8850 Bjerringbro
Germany Denmark
Declaration number Declared product / declared unit
EPD-GRU-20240274-CBA1-EN 1 PCS. of MAGNA3 (stainless steel) pump
This declaration is based on the product category rules: Scope:
Pumps for liquids and liquids with solids, 01/08/2021 The declaration applies to 1 piece of MAGNA3 (Stainless steel) pump.
(PCR checked and approved by the SVR)
The product is produced in Wahlstedt, Germany, and the life cycle
assessment is based on data collected at the production site. Production
Issue date has been modeled using annual production data from 2022.
The declaration covers the following MAGNA3 products with stainless steel
01/08/2024
pump house: MAGNA3 25-40/60/80/100/120 (threaded), MAGNA3 32-
40/60/80/100/120 (threaded), MAGNA3 32-40/60/80/100 F
(flanged),MAGNA 3 40-40/60 F (flanged).
Valid to
31/07/2029 The owner of the declaration shall be liable for the underlying information
and evidence; the IBU shall not be liable with respect to manufacturer
information, life cycle assessment data and evidences.
The EPD was created according to the specifications of EN 15804+A2. In
the following, the standard will be simplified as EN 15804.
Verification
The standard EN 15804 serves as the core PCR
Independent verification of the declaration and data according to ISO
14025:2011
Dipl.-Ing. Hans Peters internally X externally
(Chairman of Institut Bauen und Umwelt e.V.)
Florian Pronold Mrs Kim Allbury,
(Managing Director Institut Bauen und Umwelt e.V.) (Independent verifier)
1 Environmental Product Declaration - Grundfos Holding A/S - MAGNA3 25,32-40/60/80/100/120, 32-40/60/80/100 F, 40-40/60 F (Stainless steel)
Product
· solar-heating systems
Product description/Product definition The pump is suitable for thin, clean, non-aggressive and non-
The Grundfos MAGNA3 circulator pumps are designed for explosive liquids, not containing solid particles or fibres that
circulating liquids in heating systems, air conditioning and may attack the pump mechanically or chemically. In heating
cooling systems and domestic hot water systems. However, the systems, the water must meet the requirements of accepted
pump range can also be used in ground source heat pump standards on water quality in heating systems. The pumps are
systems and solar heating systems. also suitable for domestic hot-water systems.
The MAGNA3 pump is a centrifugal pump powered by an
electrical motor. It has a high-performance neodymium magnet Technical Data
rotor which increases motor efficiency and an insulation shell to The performance data of the product according to the
reduce heat loss from the stainless steel pump housing with harmonized norms, based on the harmonization provisions
threaded and flanged connections. above apply.
The declaration represents a weighted average of MAGNA3 The relevant technical specifications according to the PCR Part
pumps with identical control box and motor/pump head. The B are given in the table below.
size of the pump housing distinguishes the different pumps, Characteristics that are the same for all product groups are only
indicated in the first numbers: 25 (threaded), 32 (threaded), 32 given once. Others are given individually for all products.
F (flanged), 40 F (flanged). The average is defined based on
sales volumes.
Constructional data
Materials as well as supply chain and manufacturing processes
Name Value Unit
are identical, i.e., all cradle to gate processes (A1-A3). The
packaging is the high runner type for the included products. Frequency 50 / 60 Hz
The products are also identical in terms of distribution, Voltage 230 V
reference service life and end-of-life treatment. Pumped liquid (e.g. water) Clean Water -
Another thing that differentiates the products from each other is
Energy Efficiency Index (all, except 40-60 F) 0,18
the software which controls how the pump operates in the
Energy Efficiency Index (40-60 F) 0,19
system in which it is installed, making them fit for different
applications. This is indicated in the second numbers: 40, 60, Head max. (25,32-40, 32,40-40 F) 4 m
80, 100, 120. Hence, the use stage module B6 will change, as Head max. (25,,32-60, 32,40-60 F) 6 m
the applied scenarios for electricity consumption changes. Head max. (25,32-80, 32-80 F) 8 m
Head max. (25,32-100, 32-100 F) 10
Head max. (25,32-120) 12
Flow range max (25-40) 6,5 m3/h
For the placing on the market in the European Union/European Flow range max (25-60) 8,7 m3/h
Free Trade Association (EU/EFTA) (with the exception of Flow range max (25-80) 10,3 m3/h
Switzerland) the following legal provisions apply:
Flow range max (25-100) 11 m3/h
Machinery Directive (2006/42/EC):
Standard used: EN 809:1998 + A1:2009 Flow range max (25-120) 12,5 m3/h
Radio Equipment Directive (2014/53/EU) Flow range max (32-40, 32-40 F) 8 m3/h
Standards used:
Flow range max (32-60, 32-60 F) 10 m3/h
EN 60335-1:2012+AC:2014+A11:2014+A13:2017+A1:2019+
A14:2019+A2:2019+A15:2021, EN 60335-2-51:2003 + A1:2008 Flow range max (32-80, 32-80 F) 11,3 m3/h
+ A2:2012, EN 62233:2008. EN 55014-1:2006 + A1:2009 + Flow range max (32-100, 32-100 F) 12,3 m3/h
A2:2011, EN 55014-1:2017, EN 61000-6-2:2005, EN 61000-3- Flow range max (32-120) 12,6 m3/h
2:2014, EN 61000-3-3:2013, ETSI EN 301 489-1 V2.2.0, ETSI
Flow range max (40-40 F) 13 m3/h
EN 301 489-17 V3.2.0. ETSI EN 300 328 V2.1.1
Ecodesign Directive (2009/125/EC) Flow range max (40-60 F) 17,4 m3/h
Commission Regulation (EC) No 641/2009 and Commission Nominal capacity (25-40) 0,05 kW
Regulation (EC) No 622/2012
Nominal capacity (25-60) 0,084 kW
Standards used: EN 16297-1:2012, EN 16297-2:2012
Nominal capacity (25-80) 0,116 kW
RoHS Directive 2011/65/EU and 2015/863//EU
Standard: EN IEC 63000:2018 Nominal capacity (25-100) 0,153 kW
Nominal capacity (25-120) 0,185 kW
The CE marking takes into account the proof of conformity with Nominal capacity (32-40, 32-40 F) 0,068 kW
the respective harmonized norms based on the legal provisions
Nominal capacity (32-60, 32-60 F) 0,103 kW
above.
Nominal capacity (32-80, 32-80 F) 0,136 kW
MAGNA3 pumps are not harmonized in accordance with the
Nominal capacity (32-100, 32-100 F) 0,171 kW
CPR.
Nominal capacity (32-120) 0,182 kW
Application
Nominal capacity (40-40 F) 0,098 kW
For the application and use the respective national provisions
Nominal capacity (40-60 F) 0,185 kW
apply. The pump is designed for circulating liquids in the
following systems: Average power input values are declared in Chapter 4. LCA
· heating systems Scenarios, see table "Operational energy use (B6)".
· air-conditioning and cooling systems
· domestic water systems (only the stainless steel version) Performance data of the product according to the harmonised
· ground-source heat-pump systems standards, based on provisions for harmonisation.
2 Environmental Product Declaration - Grundfos Holding A/S - MAGNA3 25,32-40/60/80/100/120, 32-40/60/80/100 F, 40-40/60 F (Stainless steel)
Base materials/Ancillary materials The Wahlstedt production has been assessed and certified as
Base materials / Ancillary materials meeting the requirements in ISO 14001, ISO 50001, ISO 45001
and ISO 9001.
Name Value Unit
Aluminium 5,6 % Reference service life
Ceramics 0,8 % No use stage scenario which refers to the lifetime of the product
Copper 3,5 % is declared. However, to facilitate building calculations, an
estimated RSL of 10 years can be used. This is an EU
Magnet Nd 1,9 %
consensus-based estimation, referenced on page 37 in
Paper 3,6 %
Appendix 7: Lot 11 – Circulators in Buildings, prepared by AEA
PCB 4,8 % Energy & Environment for the European Commission in the
Plastics 0,5 % context of the Eco Design Directive:
Plastics, foam 1,5 %
There is no definitive information on the average circulator life
Plastics GF 12,4 %
available, there is consensus within the industry that it is at
Rubber 0,3 %
least 12 years. However, this is complicated by many factors,
Stainless steel 51,3 % including many being scrapped prematurely when e.g. the
Steel 7,1 % boiler they are connected to is replaced.
Cardboard 6,6 %
Plastic film 0,03 % From the estimated stock (140Mpa) and annual sales (14Mpa),
the average lifetime of the circulator is taken as 10 years for the
TOTAL 100 %
purposes of this study.
The RSL of the declared product is not directly influencing the
REACH results in this study, as no declared use stage scenario is
dependent on the RSL; The use stage sub-module B6 is
This product/article contains substances listed in the ECHA declared per year as required by the PCR Part B.
candidate list (date: 10.06.2022) exceeding 0.1 percentage by
mass: no
LCA: Calculation rules
Declared Unit Module A4 regards the transportation from the production site
The declared unit is 1 piece (pcs.) of MAGNA3 (Stainless steel) to the regional distribution centre, and finally to the construction
pump. and product application site. Module A5 refers to the installation
Declared unit process of the pump including the transportation of packaging
waste to the treatment site and the waste treatment of
Mass includes packaging.
packaging. The use of energy during installation is negligible for
Name Value Unit
the selected functional unit.
Declared unit 1 pce.
Mass reference 6.2 kg/pce Use stage (B1-B7):
Conversion factor [Mass/Declared Unit] 6.20 In this study, all use stage modules are assessed, though B1,
B2 and B7 are assessed to be zero. By decision no. 20170712-
Other declared units are allowed if the conversion is shown
n of the SVR, the modules B3, B4 and B5 are by default
transparently.
declared as "MNR" (module not relevant).
Contributions to operational energy use during the use stage
The weighted average product has been calculated based on
(B6) come from the electricity consumption of the product. The
the sales volumes of the included product models.
annual electricity consumption is calculated by multiplying the
average power input, which is based on a defined load profile,
with the annual running hours. For use stage (B6) European
System boundary
Average electricity grid mix has been used. These values are
This EPD is Cradle-To-Grave and Module D. The system
declared in the scenarios section.
boundaries of the EPD follow the modular approach in EN
15804.
The End-of-Life stage (C1-C4)
The End-of-Life stage (C1-C4) Modules C1-C4 refer to the End-
Production and installation (A1-A5)
of-life stage. A product reaches the end-of-life of its service life
Modules A1-A3 refer to the product stage and includes raw
when it no longer provides any functionality. This life cycle
materials extraction and processing, transportation, and the
stage includes all activities from the end-of-life of the control
manufacturing process. The product stage is included in this
valve until all materials and components are processed, reused,
study, and according to EN 15804:2019 + A2 the system
recycled, or disposed of.C1 regards the dismantling of the
boundary with nature is set to include those processes that
pump, and this module is a manual activity. C2 regards the
provide the material and energy inputs into the system and the
transport to waste processing, C3 refers to the processing
following manufacturing, transport up to the factory gate as well
(shredding) of waste for recycling, and C4 refers to waste
as the processing of waste arising from those processes. The
disposal: landfilling and incineration. The End-of-Life
assembly of the product, as well as the packaging, are also
assumption is that 95 % is collected as electronic waste, while
included in A1-A3. Wastes and losses are included in the
5 % goes to landfill. The specific amounts are shown in the
modules where they occur according to the polluter pays
scenarios section.
principle and the modular approach of EN 15804:2019+A2
3 Environmental Product Declaration - Grundfos Holding A/S - MAGNA3 25,32-40/60/80/100/120, 32-40/60/80/100 F, 40-40/60 F (Stainless steel)
Beyond system boundary (D): Land or region, in which the declared product system is
Module D refers to the burdens and benefits beyond the system manufactured, used or handled at the end of the product´s
boundaries. According to EN15804:A2+2019, module D lifespan: Europe
includes the reuse, recovery and/or recycling potentials,
expressed in net impacts and benefits. Contributions to module
Comparability
D come from waste incineration processes in A5 and C4 as well
as material (metal) recycling in C3. The specific fractions and Basically, a comparison or an evaluation of EPD data is only
net flows are shown in the scenarios section. possible if all the data sets to be compared were created
according to EN 15804 and the building context, respectively
the product-specific characteristics of performance, are taken
into account. The primary database used for background data
Geographic Representativeness is Sphera, while Ecoinvent served as a secondary database.
LCA: Scenarios and additional technical information
Name Value Unit
Characteristic product properties of biogenic carbon
Electricity consumption 25-40 114 kWh/a
The biogenic carbon content quantifies the amount of biogenic
Electricity consumption 25-60 192 kWh/a
carbon in a construction product leaving the factory gate, and it
will be separately declared for the product and for any Electricity consumption 25-80 265 kWh/a
accompanying packaging, as required from the PCR Part A. Electricity consumption 25-100 350 kWh/a
The carbon content of cardboard and paper is assumed to 0.43 Electricity consumption 25-120 423 kWh/a
kg C, meaning 43% of the paper and cardboard packaging is
Electricity consumption 32-40, 32-40 F 156 kWh/a
biogenic carbon. Overall, there is an amount of weight-%
Electricity consumption 32-60, 32-60 F 236 kWh/a
Carbon in the product leaving the factory gate and has to be
considered Electricity consumption 32-80, 32-80 F 311 kWh/a
Electricity consumption 32-100, 32-100 F 391 kWh/a
Information on describing the biogenic Carbon Content at Electricity consumption 32-120 416 kWh/a
factory gate Electricity consumption 40-40 F 224 kWh/a
Name ValueUnit Electricity consumption 40-60 F 423 kWh/a
Biogenic carbon content in accompanying kg Running hours (all products) 5.000 h/a
0.273
packaging C Average power input, 25-40 0,023 kW
Note: 1 kg of biogenic carbon is equivalent to 44/12 kg of CO2 Average power input 25-60 0,038 kW
Average power input 25-80 0,053 kW
Average power input 25-100 0,070 kW
Average power input 25-120 0,085 kW
Transport from the gate to the site (A4)
Average power input 32-40, 32-40 F 0,031 kW
Name Value Unit Average power input 32-60, 32-60 F 0,047 kW
Litres of fuel 1,7 l/100 tkm Average power input 32-80, 32-80 F 0,062 kW
Transport distance 1513 km Average power input 32-100, 32-100 F 0,078 kW
Capacity utilisation (including empty runs) 61 % Average power input 32-120 0,083 kW
Gross density of products transported 576 kg/m3 Average power input 40-40 F 0,045 kW
Wastage during distribution - % Average power input 40-60 F 0,085 kW
Installation into the building (A5) End of life (C1-C4)
Name ValueUnit Name Value Unit
Packaging waste for incineration (LDPE film) 0,02 kg Collected as mixed construction waste 5,79 kg
Packaging waste for incineration Transportation distance (C2) 100 km
0,41 kg
(Paper/Cardboard)
Aluminium for recycling 0,328 kg
An estimated RSL of 10 years can be used to facilitate building Steel for recycling 0,415 kg
calculations. This is an EU consensus-based estimation, Copper for recycling (incl. brass) 0,199 kg
referenced in Appendix 7: Lot 11 – Circulators in Buildings,
Stainless steel for recycling 3,01 kg
prepared by AEA Energy & Environment for the European
Plastics for incineration (incl. rubber) 0,719 kg
Commission in the context of the Eco Design Directive.
Electronics for incineration w/energy 0,285 kg
Reference service life
Paper for incineration 0,214 kg
Name Value Unit
Landfilling 0,62 kg
Life Span according to the manufacturer 10 a
Reuse, recovery and/or recycling potentials (D), relevant
Operational energy use (B6)
scenario information
4 Environmental Product Declaration - Grundfos Holding A/S - MAGNA3 25,32-40/60/80/100/120, 32-40/60/80/100 F, 40-40/60 F (Stainless steel)
Name Value Unit
A5, incineration w/energy recov. thermal energy 0,809 MJ
A5, incineration w/energy recov. electric energy 0,893 MJ
C3, steel for recycling (net amounts) 0,256 kg
C3, stainless steel for recycling (net amounts) 0,392 kg
C3, aluminium for recycling (net amounts) 0,004 kg
C3, copper for recycling (net amounts) 0,186 kg
C4, incineration w/energy recov. thermal energy 3,85 MJ
C4, incineration w/energy recov. electric energy 4,28 MJ
5 Environmental Product Declaration - Grundfos Holding A/S - MAGNA3 25,32-40/60/80/100/120, 32-40/60/80/100 F, 40-40/60 F (Stainless steel)
LCA: Results
Characterization model: EN 15804 - 2012+A2 - 2019, PEF. By Decision no. 20170712-n of the IBU SVR, the modules B3, B4, B5 are
marked as MNR (module not relevant) as default. The LCA results in module B6 are given on a period of one year, according to PCR
Part B. To obtain the results from module B6 over the entire life cycle, the LCA results of module B6 must be multiplied by the
estimated RSL of 10 years. The indicator results for module B6 are declared for MAGNA3 25-40. B6 indicator results for other groups
can be derived by multiplying the B6 indicator results with the following factors:
MAGNA3 25-60: 1,68; MAGNA3 25-80: 2,32; MAGNA3 25-100: 3,06; MAGNA3 25-120: 3,7;
MAGNA3 32-40, 32-40 F: 1,36; MAGNA3 32-60, 32-60 F: 2,06; MAGNA3 32-80, 32-80 F: 2,72; MAGNA3 32-100, 32-100 F: 3,42;
MAGNA3 32-120: 3,64;
MAGNA3 40-40 F: 1,95; MAGNA3 40-60 F: 3,7
DESCRIPTION OF THE SYSTEM BOUNDARY (X = INCLUDED IN LCA; MND = MODULE OR INDICATOR NOT DECLARED; MNR
= MODULE NOT RELEVANT)
Benefits and
Construction loads beyond
Product stage Use stage End of life stage
process stage the system
boundaries
la ire ta m w a Ry lp p u s tro p s n a rT g n iru tc a fu n a M e h t m o rf tro p s n a rTe tis e h t o t e ta g y lb m e s s A e s U e c n a n e tn ia M ria p e R tn e m e c a lp e R tn e m h s ib ru fe R y g re n e la n o ita re p Oe s u re ta w la n o ita re p Oe s u n o itc u rts n o c -e Dn o itilo m e d tro p s n a rT g n is s e c o rp e ts a W la s o p s iD -e s u e R-y re v o c e R-g n ilc y c e Rla itn e to p
A1 A2 A3 A4 A5 B1 B2 B3 B4 B5 B6 B7 C1 C2 C3 C4 D
X X X X X X X MNR MNR MNR X X X X X X X
RESULTS OF THE LCA - ENVIRONMENTAL IMPACT according to EN 15804+A2: 1PCS of MAGNA3 pump
Parameter Unit A1-A3 A4 A5 B1 B2 B6 B7 C1 C2 C3 C4 D
GWP-total kg CO 2 eq 4.47E+01 7.95E-01 5.9E-01 0 0 3.72E+01 0 0 4.91E-02 1.13E-01 2.55E+00 -3.06E+00
GWP-fossil kg CO 2 eq 4.57E+01 8E-01 2.32E-02 0 0 3.69E+01 0 0 4.93E-02 1.12E-01 2.24E+00 -3.05E+00
GWP-
biogenic kg CO 2 eq -1.02E+00 -1.18E-02 5.67E-01 0 0 3.21E-01 0 0 -7.3E-04 9.75E-04 3.09E-01 -3.59E-03
GWP-luluc kg CO 2 eq 4.47E-02 7.43E-03 3.59E-05 0 0 4.01E-03 0 0 4.59E-04 1.22E-05 3.75E-05 -2.55E-03
kg CFC11
ODP 3.53E-08 1.04E-13 7.19E-14 0 0 6.81E-10 0 0 6.44E-15 2.07E-12 2.83E-13 -9.66E-12
eq
AP mol H+ eq 2.51E-01 5.15E-03 1.83E-04 0 0 7.88E-02 0 0 3.18E-04 2.4E-04 6.27E-04 -2.46E-02
EP-
kg P eq 5.61E-04 2.93E-06 3.52E-08 0 0 1.38E-04 0 0 1.81E-07 4.19E-07 2.99E-06 -4.05E-06
freshwater
EP-marine kg N eq 4.96E-02 2.53E-03 6.96E-05 0 0 1.89E-02 0 0 1.56E-04 5.73E-05 2.3E-04 -2.53E-03
EP-terrestrial mol N eq 4.43E-01 2.8E-02 8.54E-04 0 0 1.97E-01 0 0 1.73E-03 5.99E-04 2.96E-03 -2.7E-02
kg NMVOC
POCP 1.24E-01 4.88E-03 1.76E-04 0 0 5.03E-02 0 0 3.01E-04 1.53E-04 6.23E-04 -8.18E-03
eq
ADPE kg Sb eq 2.87E-03 5.32E-08 8.84E-10 0 0 5.71E-06 0 0 3.28E-09 1.74E-08 2.34E-09 -5.72E-04
ADPF MJ 6.3E+02 1.09E+01 2.32E-01 0 0 7.77E+02 0 0 6.74E-01 2.36E+00 1.05E+00 -3.71E+01
m3 world eq
WDP 1.88E+01 9.7E-03 7.26E-02 0 0 8.22E+00 0 0 5.98E-04 2.5E-02 2.55E-01 -5.59E-01
deprived
GWP = Global warming potential; ODP = Depletion potential of the stratospheric ozone layer; AP = Acidification potential of land and water; EP =
Eutrophication potential; POCP = Formation potential of tropospheric ozone photochemical oxidants; ADPE = Abiotic depletion potential for non-fossil
resources; ADPF = Abiotic depletion potential for fossil resources; WDP = Water (user) deprivation potential)
RESULTS OF THE LCA - INDICATORS TO DESCRIBE RESOURCE USE according to EN 15804+A2: 1PCS of MAGNA3 pump
Parameter Unit A1-A3 A4 A5 B1 B2 B6 B7 C1 C2 C3 C4 D
PERE MJ 1.45E+02 7.96E-01 6.2E+00 0 0 4.64E+02 0 0 4.91E-02 1.41E+00 3.56E+00 -7.34E+00
PERM MJ 9.52E+00 0 -6.15E+00 0 0 0 0 0 0 0 -3.38E+00 0
PERT MJ 1.55E+02 7.96E-01 4.79E-02 0 0 4.64E+02 0 0 4.91E-02 1.41E+00 1.82E-01 -7.34E+00
PENRE MJ 6.06E+02 1.1E+01 3.87E-01 0 0 7.77E+02 0 0 6.77E-01 2.36E+00 2.59E+01 -3.72E+01
PENRM MJ 2.5E+01 0 -1.55E-01 0 0 0 0 0 0 0 -2.49E+01 0
PENRT MJ 6.31E+02 1.1E+01 2.32E-01 0 0 7.77E+02 0 0 6.77E-01 2.36E+00 1.05E+00 -3.72E+01
SM kg 4.78E+00 0 0 0 0 0 0 0 0 0 0 0
RSF MJ 0 0 0 0 0 0 0 0 0 0 0 0
NRSF MJ 0 0 0 0 0 0 0 0 0 0 0 0
FW m3 5.34E-01 8.71E-04 1.71E-03 0 0 3.75E-01 0 0 5.38E-05 1.14E-03 6E-03 -1.31E-02
PERE = Use of renewable primary energy excluding renewable primary energy resources used as raw materials; PERM = Use of renewable primary
energy resources used as raw materials; PERT = Total use of renewable primary energy resources; PENRE = Use of non-renewable primary energy
excluding non-renewable primary energy resources used as raw materials; PENRM = Use of non-renewable primary energy resources used as raw
materials; PENRT = Total use of non-renewable primary energy resources; SM = Use of secondary material; RSF = Use of renewable secondary fuels;
NRSF = Use of non-renewable secondary fuels; FW = Use of net fresh water
6 Environmental Product Declaration - Grundfos Holding A/S - MAGNA3 25,32-40/60/80/100/120, 32-40/60/80/100 F, 40-40/60 F (Stainless steel)
RESULTS OF THE LCA – WASTE CATEGORIES AND OUTPUT FLOWS according to EN 15804+A2:
1PCS of MAGNA3 pump
Parameter Unit A1-A3 A4 A5 B1 B2 B6 B7 C1 C2 C3 C4 D
HWD kg 2.68E-04 3.4E-11 5.96E-12 0 0 9.59E-08 0 0 2.1E-12 2.92E-10 5.9E-11 -2.44E-04
NHWD kg 1.74E+00 1.67E-03 1.83E-02 0 0 5.69E-01 0 0 1.03E-04 1.73E-03 6.88E-01 4.23E-01
RWD kg 1.6E-02 2.05E-05 9.85E-06 0 0 1.23E-01 0 0 1.27E-06 3.75E-04 3.54E-05 -1.65E-03
CRU kg 0 0 0 0 0 0 0 0 0 0 0 0
MFR kg 0 0 0 0 0 0 0 0 0 3.95E+00 0 0
MER kg 0 0 0 0 0 0 0 0 0 0 0 0
EEE MJ 0 0 8.93E-01 0 0 0 0 0 0 0 4.28E+00 0
EET MJ 5.51E-03 0 8.09E-01 0 0 0 0 0 0 0 3.85E+00 0
HWD = Hazardous waste disposed; NHWD = Non-hazardous waste disposed; RWD = Radioactive waste disposed; CRU = Components for re-use;
MFR = Materials for recycling; MER = Materials for energy recovery; EEE = Exported electrical energy; EET = Exported thermal energy
RESULTS OF THE LCA – additional impact categories according to EN 15804+A2-optional:
1PCS of MAGNA3 pump
Parameter Unit A1-A3 A4 A5 B1 B2 B6 B7 C1 C2 C3 C4 D
Disease
PM 3.6E-06 1.91E-08 9.63E-10 0 0 6.63E-07 0 0 1.18E-09 2.02E-09 4.37E-09 -3.94E-07
incidence
kBq U235
IR 1.91E+00 3.06E-03 1.56E-03 0 0 2.05E+01 0 0 1.89E-04 6.25E-02 5.52E-03 -2.71E-01
eq
ETP-fw CTUe 3.79E+02 7.83E+00 1.11E-01 0 0 2.16E+02 0 0 4.83E-01 7.38E-01 5.46E-01 -1.01E+01
HTP-c CTUh 3.85E-07 1.59E-10 5.52E-12 0 0 1.14E-08 0 0 9.81E-12 8.96E-11 4.61E-11 -5.51E-08
HTP-nc CTUh 5.18E-07 7.07E-09 1.49E-10 0 0 1.82E-07 0 0 4.36E-10 5.76E-09 2.71E-09 -2.25E-08
SQP SQP 2.05E+02 4.57E+00 7.35E-02 0 0 3.05E+02 0 0 2.82E-01 9.27E-01 2.07E-01 -1.11E+01
PM = Potential incidence of disease due to PM emissions; IR = Potential Human exposure efficiency relative to U235; ETP-fw = Potential comparative
Toxic Unit for ecosystems; HTP-c = Potential comparative Toxic Unit for humans (cancerogenic); HTP-nc = Potential comparative Toxic Unit for humans
(not cancerogenic); SQP = Potential soil quality index
Disclaimer 1 – for the indicator 'Potential Human exposure efficiency relative to U235'.
This impact category deals mainly with the eventual impact of low-dose ionizing radiation on human health of the nuclear fuel cycle. It
does not consider effects due to possible nuclear accidents, occupational exposure or radioactive waste disposal in underground
facilities. Potential ionizing radiation from the soil, radon and from some construction materials is also not measured by this indicator.
Disclaimer 2 – for the indicators 'abiotic depletion potential for non-fossil resources', 'abiotic depletion potential for fossil resources',
'water (user) deprivation potential, deprivation-weighted water consumption', 'potential comparative toxic unit for ecosystems', 'potential
comparative toxic unit for humans – cancerogenic', 'Potential comparative toxic unit for humans - not cancerogenic', 'potential soil
quality index'. The results of this environmental impact indicator shall be used with care as the uncertainties on these results are high
as there is limited experience with the indicator.
Disclaimer 3: JRC Technical Reports, Version 2, 2018 Page 6, for the indicator "EP-freshwater". This indicator has been calculated as
'kg P eq' as required in the characterization model EUTREND model, Struijs et al., 2009b, as implemented in ReCiPe;
References
EN 15804
Radio Equipment Directive
EN 15804:2012+A2:2019+AC:2021, Sustainability of
construction works — Environmental Product Declarations — DIRECTIVE 2014/53/EU OF THE EUROPEAN PARLIAMENT
Core rules for the product category of construction products. AND OF THE COUNCIL of 16 April 2014 on the harmonisation
of the laws of the Member States relating to the making
ISO 14025 available on the market of radio equipment
EN ISO 14025:2011, Environmental labels and declarations — Electromagnetic Compatibility (EMC) Directive
Type III environmental declarations — Principles and
procedures. DIRECTIVE 2014/30/EU OF THE EUROPEAN PARLIAMENT
AND OF THE COUNCIL of 26 February 2014 on the
IBU 2021 harmonistion of the laws of the Member States relating to
electromagnetic compatibility
Institut Bauen und Umwelt e.V.: General Instructions for the
EPD programme of Institut Bauen und Umwelt e.V., Version Ecodesign Directive
2.0, Berlin: Institut Bauen und Umwelt e.V., 2021www.ibu-
epd.com DIRECTIVE 2009/125/EC OF THE EUROPEAN PARLIAMENT
AND OF THE COUNCIL of 21 October 2009 establishing a
framework for the setting of ecodesign requirements for energy-
Standards related products
Machinery Directive EC 641/2009
DIRECTIVE 2006/42/EC OF THE EUROPEAN PARLIAMENT COMMISSION REGULATION (EC) No 641/2009 of 22 July
AND OF THE COUNCIL of 17 May 2006 on machinery 2009 implementing Directive 2005/32/EC of the European
7 Environmental Product Declaration - Grundfos Holding A/S - MAGNA3 25,32-40/60/80/100/120, 32-40/60/80/100 F, 40-40/60 F (Stainless steel)
Parliament and of the Council with regard to ecodesign electrical appliances – Safety – Part 1:General requirements
requirements for glandless standalone circulators and
glandless circulators integrated in EN 60335-2-51
products
EN 60335-2-51:2003-03 + A1:2008 + A2:2012, Household and
EC 622/2012 similar electrical appliances – Safety –Part 2-51: Particular
requirements for stationary circulation pumps for heating and
COMMISSION REGULATION (EU) No 622/2012 of 11 July service water installations
2012 amending Regulation (EC) No 641/2009 with regard to
ecodesign requirements for glandless standalone circulators EN 61000-3-2
and glandless circulators integrated in products
EN 61000-3-2:2014/2019, Electromagnetic compatibility (EMC)
DIRECTIVE 2011/65/EU – Part 3-2: Limits – Limits for harmonic current emissions
(equipment input current =16 A per phase)
DIRECTIVE 2011/65/EU OF THE EUROPEAN PARLIAMENT
AND OF THE COUNCIL of 8 June 2011 on the restriction of the EN 61000-3-3
use of certain hazardous substances es in electrical and
electronic equipment EN 61000-3-3:2013-08/ A1:2019, Electromagnetic compatibility
(EMC) – Part 3-3:
DIRECTIVE 2015/863/EU Limits – Limitation of voltage changes, voltage fluctuations and
flicker in public low voltage supply systems, for equipment with
DIRECTIVE 2015/863/EU of 31 March 2015 amending Annex II rated current <= 16 A per phase and not subject to conditional
to Directive 2011/65/EU of the European Parliament and of the connection
Council as regards the list of restricted substances
EN 61000-6-2
ETSI EN 301 489-1
EN 61000-6-2:2008/2019, Electromagnetic compatibility (EMC)
ETSI EN 301 489-1 V2.2.0, Electromagnetic Compatibility – Part 6-2: Generic standards –Immunity for industrial
(EMC) standard for radio equipment and services; Part 1: environments
Common technical requirements
EN 16297-1
ETSI EN 301 489-17
EN 16297-1:2012-10, Pumps – Rotodynamic pumps –
ETSI EN 301 489-17 V3.2.0, Electromagnetic Compatibility Glandless circulators – Part 1:
(EMC) standard for radio equipment and services; Part 17: General requirements and procedures for testing and
Specific conditions for Broadband Data Transmission Systems calculation of energy efficiency index (EEI)
ETSI EN 300 328 V2.1.1 EN 16297-2
ETSI EN 300 328 V2.1.1, Wideband transmission systems; EN 16297-2:2012-10, Pumps – Rotodynamic pumps –
Data transmission equipment operating in the 2,4 GHz ISM Glandless circulators – Part 2: Calculation of energy efficiency
band and using wide band modulation techniques index (EEI) for standalone circulators
EN 809 EN 16297-3
EN 809:1998-10 + A1:2009, Pumps and pump units for liquids - EN 16297-3:2012, Pumps – Rotodynamic pumps –Glandless
Common safety requirements circulators – Part 3: Energy efficiency index (EEI) for circulators
integrated in products
EN 55014-1
ISO 14001
EN 55014-1:2017, Electromagnetic compatibility –
Requirements for household appliances, electric tools and EN ISO 14001:2015-09, Environmental management systems -
similar apparatus – Part 1: Emission Requirements with guidance for use
EN 55014-2 ISO 14025
EN 55014-2:2015, Electromagnetic compatibility – DIN EN /ISO 14025:2011-10, Environmental labels and
Requirements for household appliances, electric tools and declarations — Type III environmental declarations —
similar apparatus – Part 2: Immunity – Product family standard Principles and procedures
(CISPR 14-2:2015)
EN 15804
EN 50581:2012
EN 15804:2012-04+A1 2013, Sustainability of construction
EN 50581:2012, Technical documentation for the assessment works — Environmental Product Declarations — Core rules for
of electrical and electronic products with respect to the the product category of construction products
restriction of hazardous substances
PCR Part A
EN 60335-1
Institut Bauen und Umwelt e.V., Berlin (pub.): Product Category
EN 60335-1:2012/A11:2014/A13:2017, Household and similar Rules for Building-Related Products and Services, Product
8 Environmental Product Declaration - Grundfos Holding A/S - MAGNA3 25,32-40/60/80/100/120, 32-40/60/80/100 F, 40-40/60 F (Stainless steel)
Category Rules for Construction Products from the range of ECHA candidate list
Environmental Product Declarations of Institut Bauen und
Umwelt (IBU), Part A: Calculation Rules for the Life Cycle Candidate List of substances of very high concern (SVHCs) for
Assessment and Requirements on the Project Report, Version authorisation, European Chemicals Agency (ECHA), Helsinki,
1.3. Finland
PCR Part B EUTREND model
Struijs et al., 2009b AEA Energy & Environment
Institut Bauen und Umwelt e.V., Berlin (pub.): Product Category Circulators in Buildings
Rules for Building-Related Products and Services, Product
Category Rules for Construction Products from the range of Ecoinvent
Environmental Product Declarations of Institut Bauen und Ecoinvent v3.9.1
Umwelt (IBU), Part B: Requirements on the EPD for Pumps for
liquids and liquids with solids, Version 1.0 (2018) LCA for Experts
10.7.1.28 Schema 8007
Further references
CPR REACH Regulation (EC) No 1907/2006 of the European
Parliament and of the Council of 18 December 2006 concerning
REGULATION (EU) No 305/2011 OF THE EUROPEAN the Registration, Evaluation, Authorisation and Restriction of
PARLIAMENT AND OF THE COUNCIL of 9 March 2011 laying Chemicals (REACH) (Status: 27.06.2018)
down harmonised conditions for the marketing of construction
products and repealing Council Directive 89/106/EEC SVR
CML 2001 Advisory Board (formerly SVA)
Impact assessment characterization factors Institute of Decision no.
Environmental Sciences, Leiden University, Netherlands 20170712-n
9 Environmental Product Declaration - Grundfos Holding A/S - MAGNA3 25,32-40/60/80/100/120, 32-40/60/80/100 F, 40-40/60 F (Stainless steel)
Publisher
Institut Bauen und Umwelt e.V. +49 (0)30 3087748- 0
Hegelplatz 1 info@ibu-epd.com
10117 Berlin www.ibu-epd.com
Germany
Programme holder
Institut Bauen und Umwelt e.V. +49 (0)30 3087748- 0
Hegelplatz 1 info@ibu-epd.com
10117 Berlin www.ibu-epd.com
Germany
Author of the Life Cycle Assessment
Grundfos Holding A/S +45 87501400
Poul Due Jensens Vej 7 LCA_EPD@grundfos.com
8850 Bjerringbro www.grundfos.com
Denmark
Owner of the Declaration
Grundfos Holding A/S +45 87501400
Poul Due Jensens Vej 7 LCA_EPD@grundfos.com
8850 Bjerringbro www.grundfos.com
Denmark
10 Environmental Product Declaration - Grundfos Holding A/S - MAGNA3 25,32-40/60/80/100/120, 32-40/60/80/100 F, 40-40/60 F (Stainless steel)
