ENVIRONMENTAL PRODUCT DECLARATION
as per ISO 14025 and EN 15804+A2
Owner of the Declaration dormakaba International Holding GmbH
Publisher Institut Bauen und Umwelt e.V. (IBU)
Programme holder Institut Bauen und Umwelt e.V. (IBU)
Declaration number EPD-DOR-20210194-CBC7-EN
Issue date 01.10.2021
Valid to 30.09.2026
Serrated Double Cylinder - pextra Q, pextra+, pextra, AP 2000
dormakaba
www.ibu-epd.com | https://epd-online.com
General Information
dormakaba Serrated Double Cylinder - pextra Q, pextra+,
pextra, AP 2000
Programme holder Owner of the declaration
IBU – Institut Bauen und Umwelt e.V. dormakaba International Holding GmbH
Hegelplatz 1 DORMA Platz 1
10117 Berlin 58256 Ennepetal
Germany Germany
Declaration number Declared product / declared unit
EPD-DOR-20210194-CBC7-EN 1 piece of the product: one (1) dormakaba pextra Q mechanical key
system, consisting of the following items:
- one (1) pextra Q double cylinder
- three (3) pextra Q serrated keys
- one (1) cylinder mounting screw
- one (1) security card
- one (1) user manual
- packaging
This declaration is based on the product category rules: Scope:
Building Hardware products, 01.08.2021 This declaration is a specific product declaration for the pextra Q double
(PCR checked and approved by the SVR) cylinder including three keys. This Environmental Product Declaration is
also representative for the systems pextra+, pextra and AP 2000. The
underlying life cycle assessment is based on the entire life cycle of this
Issue date specific mechanical key system. Data represents the year 2021. The
products are manufactured at the dormakaba production facilities in
01.10.2021
Herzogenburg, Austria.
The owner of the declaration shall be liable for the underlying information
and evidence; the IBU shall not be liable with respect to manufacturer
Valid to
information, life cycle assessment data and evidences.
30.09.2026
The EPD was created according to the specifications of EN 15804+A2. In
the following, the standard will be simplified as EN 15804.
Verification
The standard EN 15804 serves as the core PCR
Independent verification of the declaration and data according to ISO
14025:2011
internally X externally
Dipl.-Ing. Hans Peters
(Chairman of Institut Bauen und Umwelt e.V.)
Florian Pronold Dr.-Ing. Wolfram Trinius,
(Managing Director Institut Bauen und Umwelt e.V.) (Independent verifier)
1 Environmental Product Declaration - dormakaba - Serrated Double Cylinder - pextra Q, pextra+, pextra, AP 2000
Product
limitless application options are possible.
Product description/Product definition
Information about the enterprise Technical Data
dormakaba stands for a broad offering of products, solutions pextra Q, pextra+, pextra and AP2000 are a high-performance
and services for smart and secure access to buildings and locking systems, which fulfills even the most challenging
rooms from a single source. requirements. They offer exceptional security thanks to:
• Five to seven pins with additional side elements
Product description/ Product definition
• Wide range of different key profiles
pextra Q, pextra+, pextra and AP2000 are serrated master key
• Cylinder bodies are made of brass
systems representing the high-quality segment.
• Keys are made of nickel silver
Furthermore, pextra Q and pextra+ are patented and offer legal
protection against commercial imitation. Duplicate keys are only
Furthermore for pextra Q and pextra+:
made by dormakaba itself or by authorized partners and require
identification by means of a security card. • Key protected by the patented single or double branch
groove
The main production site of dormakaba serrated key systems • Technical protection of the patent with an optional active
cylinders/keys and parts is in Herzogenburg, Austria. Finished pin in the cylinder
cylinders and keys are manufactured either directly in the Delivery status:
factory or by authorised dealers. The product range consists of
factory-made profiles and dealer profiles. One (1) serial standard double cylinder includes three (3) keys,
Whilst cylinders and keys with factory made profiles are a mounting-screw, a user-manual and a security card. Including
manufactured in our factory, keys with dealer profiles can also the packaging the cylinder will be supplied with a weight of
be finalized directly with authorised dealers. 0,264 kg.
Base materials/Ancillary materials
For placing the mechanical key systems on the market in the
The material composition of the product is the following:
European Union/European Free Trade Association (EU/EFTA,
with the exception of Switzerland) the following legal provisions
apply:
All systems are classified according to the European locking
cylinder standards EN1303 and DIN18252. While the basic
cylinder configuration already fulfils the attack resistance class
C, the highest protection grade D can be achieved with an
additional steel reinforcemnt bar or a scarificial breaking slot.
These figures are also representative for the serrated systems
pextra and AP2000.
The cylinders and keys contain partial articles which contain
substances listed in the Candidate List of REACH Regulation
*locking security 5 for 5-pin, 6 for 6- and 7-pin 1907/2006/EC (date: 19.01.2021) exceeding 0.1 percentage by
mass: yes
dormakaba mechanical cylinders fulfill the material
• Lead (Pb): 7439-92-1 (CAS-No.) is included in some of
requirements given within the Directive RoHS 2011/65/EU. In
the alloys used. The concentration of lead in each
addition, cylinders are fire protection tested according to EN
individual alloy does not exceed 4.0% (by mass).
1634-1 and EN 1634-2.
The candidate list can be found on the /ECHA/ website
One speciality about the serrated key systems is that a high
address:
degree of components can be used throughout different
https://echa.europa.eu/de/home.
systems, an example would be the cylinder housing itself or the
pins.
This helps to reduce stock and increases the efficiency when it Reference service life
comes to transportation and production.
The life cycle of a lock cylinder is about 10-15 years, depending
on the application and frequency of use. The cylinders are
Application
tested to 100,000 locking cycles minimum (EN1303). This
The dormakaba serrated cylinder range with pextra Q, pextra+,
corresponds to approximately 15-18 locking cycles per day for
pextra and AP2000 can be used in both residential as well as in
15 years.
the commercial segment in small and simple as well as in large
and complex applications, thanks to its versatility. Nearly
LCA: Calculation rules
Name Value Unit
Declared Unit
Declared unit 1 piece/product
The declared unit is 1 piece of the product: pextra Q
Mass of declared product including
Declared unit packaging 0.264 kg
2 Environmental Product Declaration - dormakaba - Serrated Double Cylinder - pextra Q, pextra+, pextra, AP 2000
The end-of-life stage includes:
System boundary — C1, de-construction, demolition:
The type of EPD is according to EN 15804: — C2, transport to waste processing;
"cradle to gate with options, modules C1–C4, and module D". — C3, waste processing for reuse, recovery and/or recycling;
The following modules are declared: A1-A3, C1-C4, D and — C4, disposal; including provision and all transport, provision
additional modules: A4 + A5 Production - Module A1-A3 of all materials, products and related energy and water use.
The product stage includes: Module D (Benefits and loads beyond the system boundary)
includes:
— A1, raw material extraction, processing and mechanical — D, recycling potentials, expressed as net impacts and
treatments, processing of secondary material input (e.g. benefits.
recycling processes),
— A2, transport to the manufacturer, Geographic Representativeness
— A3, manufacturing and assembly including provision of all Land or region, in which the declared product system is
materials, products and energy, as well as waste processing up manufactured, used or handled at the end of the product´s
to the end-of waste state. lifespan: Austria
Construction stage - Modules A4-A5
Comparability
The construction process stage includes:
— A4, transport to the building site; Basically, a comparison or an evaluation of EPD data is only
— A5, installation into the building; including provision of all possible if all the data sets to be compared were created
materials, products and energy, as well as waste processing up according to EN 15804 and the building context, respectively
to the end-ofwaste state or disposal of final residues during the the product-specific characteristics of performance, are taken
construction process stage. into account. Background database: GaBi ts
software, SP40.
End-of-life stage– Modules C1-C4 and D
LCA: Scenarios and additional technical information
Characteristic product properties of biogenic carbon In case a reference service life according to applicable ISO
Information on describing the biogenic Carbon Content at standards is declared then the assumptions and in-use
factory gate conditions underlying the determined RSL shall be declared. In
addition, it shall be stated that the RSL applies to the reference
Name ValueUnit
conditions only.
Biogenic carbon content in accompanying kg
0.01
packaging C
The same holds for a service life declared by the manufacturer.
Corresponding information related to in-use conditions needs
The following technical scenario information is required for the not be provided if a service life taken from the list of service life
declared modules. by BNB is declared.
Transport to the building site (A4)
End of life (C1-C4)
Name Value Unit
C1: The product dismantling from the building is done manually
Litres of fuel (per piece) 0.0015l/100km
without environmental burden.
Transport distance plane 124 km
Name Value Unit
Transport distance truck 812 km
Collected separately waste type 0.233 kg
Capacity utilisation (including empty runs)
51 % Recycling 0.224 kg
average
Energy recovery 0.00948 kg
The product is transported via plane and truck. The main
distribution regions are Europe and Asia. In order to allow The product is disassembled in a recycling process.
scaling to a specific point of installation 100 km are declared as Material recycling is then assumed for the metals. The plastic
well. components are assumed to be incinerated with energy
recovery.
Installation into the building (A5)
Reuse, recovery and/or recycling potentials (D), relevant
Name Value Unit scenario information
Waste packaging (paper) 0,031 kg Collection rate is 100%.
3 Environmental Product Declaration - dormakaba - Serrated Double Cylinder - pextra Q, pextra+, pextra, AP 2000
LCA: Results
DESCRIPTION OF THE SYSTEM BOUNDARY (X = INCLUDED IN LCA; MND = MODULE OR INDICATOR NOT DECLARED; MNR
= MODULE NOT RELEVANT)
Benefits and
Construction loads beyond
Product stage Use stage End of life stage
process stage the system
boundaries
la ire ta m w a Ry lp p u s tro p s n a rT g n iru tc a fu n a M e h t m o rf tro p s n a rTe tis e h t o t e ta g y lb m e s s A e s U e c n a n e tn ia M ria p e R tn e m e c a lp e R tn e m h s ib ru fe R y g re n e la n o ita re p Oe s u re ta w la n o ita re p Oe s u n o itc u rts n o c -e Dn o itilo m e d tro p s n a rT g n is s e c o rp e ts a W la s o p s iD -e s u e R-y re v o c e R-g n ilc y c e Rla itn e to p
A1 A2 A3 A4 A5 B1 B2 B3 B4 B5 B6 B7 C1 C2 C3 C4 D
X X X X X MND MND MNR MNR MNR MND MND X X X X X
RESULTS OF THE LCA - ENVIRONMENTAL IMPACT according to EN 15804+A2: 1 piece, Serrated double cylinder - pextra Q,
pextra+, pextra, AP 2000
Parameter Unit A1-A3 A4 A5 C1 C2 C3 C4 D
GWP-total kg CO 2 eq 6.91E-01 1.21E-01 4.4E-02 0 1E-03 2.4E-02 0 -2.14E-01
GWP-fossil kg CO 2 eq 6.82E-01 1.18E-01 1E-03 0 9.75E-04 2.4E-02 0 -2.14E-01
GWP-biogenic kg CO 2 eq 7.47E-03 2E-03 4.3E-02 0 4.51E-05 5.61E-07 0 8.87E-04
GWP-luluc kg CO 2 eq 1.27E-03 2.61E-06 7.23E-07 0 2.32E-08 1.36E-06 0 -4.67E-04
ODP kg CFC11 eq 3.49E-13 1.01E-17 7.92E-18 0 1.03E-19 1.22E-17 0 -1.07E-15
AP mol H+ eq 6.37E-03 3.39E-04 1.23E-05 0 9.76E-07 4.29E-06 0 -3E-03
EP-freshwater kg P eq 2.26E-06 2.17E-08 1.55E-09 0 2.09E-10 1.94E-09 0 -1.75E-07
EP-marine kg N eq 4.87E-04 1.45E-04 4.44E-06 0 3.11E-07 9.67E-07 0 -1.76E-04
EP-terrestrial mol N eq 5.09E-03 2E-03 5.54E-05 0 3.45E-06 1.95E-05 0 -2E-03
kg NMVOC
POCP 1.29E-03 4.17E-04 1.18E-05 0 8.78E-07 2.68E-06 0 -6.52E-04
eq
ADPE kg Sb eq 2.46E-04 3.43E-09 1.25E-10 0 2.92E-11 1.67E-10 0 -1.34E-04
ADPF MJ 8.62E+00 1.63E+00 1.4E-02 0 1.4E-02 1.1E-02 0 -2.29E+00
m3 world eq
WDP 2.43E-01 2E-04 5E-03 0 1.91E-06 2E-03 0 -1.31E-01
deprived
GWP = Global warming potential; ODP = Depletion potential of the stratospheric ozone layer; AP = Acidification potential of land and water; EP =
Eutrophication potential; POCP = Formation potential of tropospheric ozone photochemical oxidants; ADPE = Abiotic depletion potential for non-fossil
resources; ADPF = Abiotic depletion potential for fossil resources; WDP = Water (user) deprivation potential)
RESULTS OF THE LCA - INDICATORS TO DESCRIBE RESOURCE USE according to EN 15804+A2: 1 piece, Serrated double
cylinder - pextra Q, pextra+, pextra, AP 2000
Parameter Unit A1-A3 A4 A5 C1 C2 C3 C4 D
PERE MJ 4.06E+00 4E-03 3.75E-01 ND 4.36E-05 3E-03 0 -3.93E-01
PERM MJ 3.72E-01 0 -3.72E-01 ND 0 0 0 0
PERT MJ 4.44E+00 4E-03 3E-03 ND 4.36E-05 3E-03 0 -3.93E-01
PENRE MJ 8.48E+00 1.64E+00 1.4E-02 ND 1.4E-02 1.62E-01 0 -2.29E+00
PENRM MJ 1.51E-01 0 0 ND 0 -1.51E-01 0 0
PENRT MJ 8.63E+00 1.64E+00 1.4E-02 ND 1.4E-02 1.1E-02 0 -2.29E+00
SM kg 1.81E-01 0 0 ND 0 0 0 0
RSF MJ 0 0 0 ND 0 0 0 0
NRSF MJ 0 0 0 ND 0 0 0 0
FW m3 6E-03 8.27E-06 1.28E-04 ND 7.82E-08 5.9E-05 0 -2E-03
PERE = Use of renewable primary energy excluding renewable primary energy resources used as raw materials; PERM = Use of renewable primary
energy resources used as raw materials; PERT = Total use of renewable primary energy resources; PENRE = Use of non-renewable primary energy
excluding non-renewable primary energy resources used as raw materials; PENRM = Use of non-renewable primary energy resources used as raw
materials; PENRT = Total use of non-renewable primary energy resources; SM = Use of secondary material; RSF = Use of renewable secondary fuels;
NRSF = Use of non-renewable secondary fuels; FW = Use of net fresh water
RESULTS OF THE LCA – WASTE CATEGORIES AND OUTPUT FLOWS according to EN 15804+A2:
1 piece, Serrated double cylinder - pextra Q, pextra+, pextra, AP 2000
Parameter Unit A1-A3 A4 A5 C1 C2 C3 C4 D
HWD kg 3.62E-08 1.57E-10 2.05E-11 ND 1.34E-12 4.26E-11 0 -1.25E-08
NHWD kg 1.45E-01 1.66E-04 1E-03 ND 1.42E-06 3E-03 0 -7.4E-02
RWD kg 3.58E-04 1.51E-06 7.29E-07 ND 1.49E-08 4.15E-07 0 -2.56E-05
CRU kg 0 0 0 ND 0 0 0 0
MFR kg 0 0 0 ND 0 2.24E-01 0 0
MER kg 0 0 0 ND 0 0 0 0
EEE MJ 8.6E-02 0 6.6E-02 ND 0 0 0 0
EET MJ 1.56E-01 0 1.21E-01 ND 0 0 0 0
4 Environmental Product Declaration - dormakaba - Serrated Double Cylinder - pextra Q, pextra+, pextra, AP 2000
HWD = Hazardous waste disposed; NHWD = Non-hazardous waste disposed; RWD = Radioactive waste disposed; CRU = Components for re-use;
MFR = Materials for recycling; MER = Materials for energy recovery; EEE = Exported electrical energy; EET = Exported thermal energy
RESULTS OF THE LCA – additional impact categories according to EN 15804+A2-optional:
1 piece, Serrated double cylinder - pextra Q, pextra+, pextra, AP 2000
Parameter Unit A1-A3 A4 A5 C1 C2 C3 C4 D
Disease
PM 5.1E-08 1.19E-09 6.82E-11 ND 5.13E-12 5.47E-11 0 -2.8E-08
incidence
IR kBq U235 eq 4.41E-02 2.1E-04 1.13E-04 ND 2.12E-06 3.74E-05 0 -5E-03
ETP-fw CTUe 5.57E+00 1.16E+00 7E-03 ND 1E-02 4E-03 0 -1.94E+00
HTP-c CTUh 1.02E-09 2.18E-11 3.48E-13 ND 1.84E-13 3.63E-13 0 -1.5E-10
HTP-nc CTUh 2.44E-08 1.07E-09 1.51E-11 ND 7.89E-12 3.68E-11 0 -1.2E-08
SQP SQP 1.13E+01 4E-03 4E-03 ND 3.55E-05 3E-03 0 -2.08E+00
PM = Potential incidence of disease due to PM emissions; IR = Potential Human exposure efficiency relative to U235; ETP-fw = Potential comparative
Toxic Unit for ecosystems; HTP-c = Potential comparative Toxic Unit for humans (cancerogenic); HTP-nc = Potential comparative Toxic Unit for humans
(not cancerogenic); SQP = Potential soil quality index
Disclaimer 1 – for the indicator “Potential Human exposure efficiency relative to U235”. This impact category deals mainly with the
eventual impact of low-dose ionizing radiation on human health of the nuclear fuel cycle. It does not consider effects due to possible
nuclear accidents, occupational exposure or radioactive waste disposal in underground facilities. Potential ionizing radiation from the
soil, radon and from some construction materials is also not measured by this indicator.
Disclaimer 2 – for the indicators “abiotic depletion potential for non-fossil resources”, “abiotic depletion potential for fossil resources”,
“water (user) deprivation potential, deprivation-weighted water consumption”, “potential comparative toxic unit for ecosystems”,
“potential comparative toxic unit for humans – cancerogenic”, “Potential comparative toxic unit for humans - not cancerogenic”,
“potential soil quality index”. The results of this environmental impact indicator shall be used with care as the uncertainties on these
results are high as there is limited experience with the indicator.
References
DIN 18252
DIN 18252: 2018, Profile cylinders for door locks – Terminology, European Chemicals Agency (ECHA)
dimensions, requirements, test methods and marking https://echa.europa.eu/de/
DIN EN 1303 Further References
DIN EN 1303: 2015, Building Hardware - Cylinders for locks -
Requirements and test methods IBU
Institut Bauen und Umwelt e.V.:
DIN EN 1634-1 General Instructions for the EPD Programme of Institut Bauen
DIN EN 1634-1:2018, Fire resistance and smoke control tests und Umwelt e.V. Version 2.0., Berlin: Institut Bauen und Umwelt
for door and shutter assemblies, openable windows and e.V., 2021.
elements of building hardware www.ibu-epd.com
DIN EN 1634-2 GaBi ts software
DIN EN 1634-2:2009, Fire resistance and smoke control tests Sphera Solutions GmbH Gabi Software System and Database
for door, shutter and openable window assemblies and for Life Cycle Engineering 1992-2020 Version 10.0.0.71
elements of building hardware University of Stuttgart Leinfelden-Echterdingen
DIN EN ISO 14025 GaBi ts documentation
DIN EN ISO 14025:2011, Environmental labels and GaBi life cycle inventory data documentation (https://www.gabi-
declarations — Type III environmental declarations - Principles software.com/support/gabi/gabidatabase- 2020-lci-
and procedures. documentation/).
EN 15804 LCA-tool dormakaba
EN 15804:2019+A2, Sustainability of construction works — LCA tool, version 1.0.
Environmental Product Declarations — Core rules for the Developed by Sphera Solutions GmbH
product category of construction products.
PCR Part A
REACH Regulation PCR – Part A: Calculation Rules for the Life Cycle Assessment
REACH Regulation (EC) No 1907/2006 of the European and Requirements on the Project Re-port according to EN
Parliament and of the Council on the Registration, Evaluation, 15804+A2:2019, Version 1.0, Institut Bauen und Umwelt e.V.,
Authorisation and Restriction of Chemicals. www.ibu-epd.com.
RoHS 2011/65/EU PCR Part B
RoHS 2011/65/EU, Directive on the restriction of the use of PCR – Part B: Requirements on the EPD for Building Hardware
certain hazardous substances in electrical and electronic Products, version 08/2021, Institut Bauen und Umwelt e.V.,
equipment. www.ibu-epd.com.
5 Environmental Product Declaration - dormakaba - Serrated Double Cylinder - pextra Q, pextra+, pextra, AP 2000
Publisher
Institut Bauen und Umwelt e.V. +49 (0)30 3087748- 0
Hegelplatz 1 info@ibu-epd.com
10117 Berlin www.ibu-epd.com
Germany
Programme holder
Institut Bauen und Umwelt e.V. +49 (0)30 3087748- 0
Hegelplatz 1 info@ibu-epd.com
10117 Berlin www.ibu-epd.com
Germany
Author of the Life Cycle Assessment
Sphera Solutions GmbH +49 711 341817-0
Hauptstraße 111- 113 info@sphera.com
70771 Leinfelden-Echterdingen www.sphera.com
Germany
Owner of the Declaration
dormakaba International Holding GmbH +49 2333 793-0
DORMA Platz 1 info.de@dormakaba.com
58256 Ennepetal www.dormakaba.com
Germany
6 Environmental Product Declaration - dormakaba - Serrated Double Cylinder - pextra Q, pextra+, pextra, AP 2000
