ENVIRONMENTAL PRODUCT DECLARATION
as per ISO 14025 and EN 15804+A2
Owner of the Declaration Holcim (Germany) GmbH
Programme holder Institut Bauen und Umwelt e.V. (IBU)
Publisher Institut Bauen und Umwelt e.V. (IBU)
Declaration number EPD­HOC­20220204­IBD1­EN
Issue date 21.09.2022
Valid to 20.09.2027
Airium™ Spray: cement-based insulation foam
Holcim (Germany) GmbH
www.ibu-epd.com | https://epd-online.com
Umwelt Produktdeklaration Name des Herstellers – Name des Produkts
1. General Information
Holcim (Germany) GmbH Airium cement-based insulation
foam
Programme holder Owner of the declaration
IBU – Institut Bauen und Umwelt e.V. Holcim (Deutschland) GmbH
Hegelplatz 1 Willy­Brandt­Straße 69
10117 Berlin 20457 Hamburg
Germany
Declaration number Declared product / declared unit
EPD­HOC­20220204­IBD1­EN 1 m3 of Airium™ cement­based insulation foam with an
average wet density of 130 kg/m3 and an average dry
density of 100 kg/m3.
The declared values can also be scaled to Airium™
cement­based insulation foam with an average wet
density of 300 kg/m3 and an average dry density of 250
kg/m3.
This declaration is based on the product Scope:
category rules: Airium™ Spray is a cement­based insulation foam
cement­based foams, 05.2020 produced on site by mixing two components: a dry
(PCR checked and approved by the SVR) slurry made with premix and water and a diluted
solution of hydrogen peroxide. The life cycle
assessment is based on components produced in
Issue date
different plants and on­site production data. The
21.09.2022
premix is produced by HASIT (plant located in Kissing,
Germany) with cement produced by Holcim Germany
Valid to (plant located in Dotternhausen, Germany), and
20.09.2027 additives produced by other suppliers. The diluted
solution of hydrogen peroxide is produced by Solvay
(the foreground data are primary production data from
Solvay industrial sites in Europe).
The owner of the declaration shall be liable for the
underlying information and evidence; the IBU shall not
be liable with respect to manufacturer information, life
cycle assessment data and evidences.
The EPD was created according to the specifications
of EN 15804+A2. In the following, the standard will be
simplified as EN 15804.
Verification
The standard EN 15804 serves as the core PCR
Independent verification of the declaration and data
according to ISO 14025:2011
Dipl. Ing. Hans Peters internally x externally
(chairman of Institut Bauen und Umwelt e.V.)
Dr. Alexander Röder Dr. Matthew Fishwick
(Managing Director Institut Bauen und Umwelt e.V.)) (Independent verifier)
2. Product
2.1 Product description/Product definition on vertical surfaces. Airium™ Spray, within a full
Airium™ Spray is an insulating technology that system approach developed through a partnership
improves the energy efficiency of buildings as part of between Holcim and HASIT Group, aims to fulfil all
External Thermal Insulation Composite Systems core requirements of ETICS in new­build and in
(ETICS). Airium™ Spray is generated via a continuous renovation projects:
chemical foaming reaction by mixing a cement­based  it is an efficient insulator in cold and hot
dry slurry and a diluted solution of hydrogen peroxide weather. It also has a superior thermal phase
with a dedicated equipment.
shift (14 hours) than wool and polystyrene
alternatives;
Airium™ Spray is the first mineral foam to offer a top­
tier insulating performance and which can be applied  it is ranked A1 and is fully fire resistant;
2 Environmental Product Declaration HOLCIM Deutschland – Airium cement­based insulation foam
 it contains no harmful fibres, emits no volatile Performance data of the product with respect to its
organic compounds (VOCs) and is a characteristics in accordance with the relevant
technical provision (no CE­marking).
breathable material that limits the risk of
mould;
2.4 Delivery status
 it provides a continuous insulation layer with Airium™ Spray is a cement­based insulation foam
no thermal bridges; produced on site with an average wet density of 130
 it insulates efficiently over time as it is kg/m3 and an average dry density of 100 kg/m3.
dimensionally stable and does not settle or Several layers can be applied to reach the thermal
resistance targeted.
sag;
 it accelerates the time required to place
2.5 Base materials/Ancillary materials
insulation on site by a factor of 2 while Airium™ Spray is produced on site by mixing two
diminishing waste and storage space required components: a dry slurry made with premix and water
on site; (25­35 %w of the premix) and a diluted solution of
 it is resistant to insects or rodents; hydrogen peroxide. When both components are mixed,
water and oxygen are generated in the slurry to obtain
 it is highly insulating over time and recyclable,
the cement­based foam.
in cement, in concrete or in Airium™ with no
separation phase. The composition of the premix powder is indicated as
follows:
 cement 70 ­ 80 w%
 limestone filler: 10 ­ 20 w%
For the use and application of the product the  stabilizer: 3 ­ 7 w%
respective national provisions at the place of use
 water reducing agent: < 1 w%
apply, in Germany for example the building codes of
 catalyst: < 1 w%
the federal states and the corresponding national
specifications.  accelerator: < 0,1 w%
 PP fibres: < 0,1 w%
2.2 Application
Airium™ Spray is a cement­based insulation foam
The diluted solution of hydrogen peroxide has a H O
produced on site and applied by hand. It can be used 2 2
concentration of <8 w%.
for retrofitting and new construction. The insulation
after hardening can be covered with claddings or
1) This product/article/at least one partial article
plastered with specialized mortar and components
contains substances listed in the ECHA candidate list
used for ETICS.
(date: 15.03.2022) exceeding 0.1 percentage by mass:
For use in old and new building insulation:
 no
 As system component in the thermal
insulation composite system (ETICS)
2) This product/article/at least one partial article
 Interior and exterior insulation of outside walls
contains other carcinogenic, mutagenic or reprotoxic
 Double­wall masonry
(CMR) substances in categories 1A or 1B which are
 Wall cavity insulation not on the ECHA candidate list, exceeding 0.1
 Ventilated curtain facades percentage by mass:
 no
2.3 Technical Data 3) Biocide products were added to this construction
product or it has been treated with biocide products
(this then concerns a treated product as defined by the
Constructional Data (EU) Ordinance on Biocide Products No. 528/2012):
Name Value Unit  no
Gross density (EN 1602) 90 ­ 110 kg/m3
Dimensional stability (EN 1604) ­0.3 %
0.0415 ­
Thermal conductivity (EN 12667) W/(mK)
0.0445
2.6 Manufacture
Specific heat capacity (EN 10456) 1 kJ/kgK
The raw materials are stored at the manufacturing
Water vapour diffusion resistance
3 ­ plant in silos or IBCs. From the silos, the raw materials
factor (ISO 12572)
are dosed and intensely mixed according to the
flexural stress mean value) (EN
25 kPa formulation. The mixture is then packaged and shipped
998­1)
in packages or in a silo.
Melting point > 1200 °C
Tensile strenght (EN 998­1) 0,007 N/mm^2
The manufacturing process of the premix is illustrated
Moisture content after conditioning
14,5 % using the following graphic.
at 23 °C / 80 % R.H (EN 1602)
Reaction to fire (EN 13501)) A1 ­
Compressive strength (mean
0,07 N/mm^2
value) (EN 998­1)
3 Environmental Product Declaration HOLCIM Deutschland – Airium cement­based insulation foam
2.12 Reference service life
A reference service life according to the ISO 15686
series of standards is not declared.
When used as intended, the service life of
the insulation boards is <50 years according to
the Bundesinstitut für Bau­, Stadt­ und
Raumforschung (BBSR 2017) table “Service life of
components for life cycle analyses according to the
assessment system for sustainable building (BNB).
Cement­based insulation foams are not directly
exposed to environmental conditions; relevant effects
due to ageing cannot be observed over the reference
service life.
2.7 Environment and health during
manufacturing 2.13 Extraordinary effects
No environmental or health protection measures other
than those specified by law are necessary. Fire
As a mineral­based material, Airium™ cement­based
2.8 Product processing/Installation insulation foam is not inflammable.
On the construction site, the components are mixed
and water is added to produce the insulation foam Name Value Unit
ready to be applied. The product is then Building material class A1 ­
pumped/sprayed to the area of application.
Water
2.9 Packaging As a mineral­based material, Airium™ cement­based
For larger applications, the two components of Airium insulation foam is not sensitive to the influence of
cement­based insulation foam are brought to the water, e.g., related to flooding.
construction site in a multi­use dual silo.
For smaller applications, the dry slurry is packed in Mechanical destruction
paper bags including a PE­foil, which can be used for Not relevant.
energy recovery.
2.14 Re-use phase
After crushing and sieving the insulated wall, Airium™
2.10 Condition of use cement­based insulation foam powder can be recycled
During service life, Airium cement­based insulation and used as a filler material in concrete or mortar
foam re­absorbs (carbonation) CO 2 emitted during production, substituting e.g., from milled limestone.
cement production (calcination).
2.15 Disposal
For details, see clause 4. In case recycling is not feasible, Airium™ cement­
based foam can be disposed of in an inert material
2.11 Environment and health during use landfill together with other mineral de­construction
The product is stable during use; its composition does waste.
not change, except for the uptake of CO
2
(carbonation). Waste code according to the European Waste Index:
17 01 01 concrete
The product does not contain harmful substances that
could affect health or the environment. 2.16 Further information
You can find more information about Airium™ cement­
based insulation foam under: www.airium.com
3. LCA: Calculation rules
3.1 Declared Unit Modules A1-A3 contain the production of the dry
The declared unit is 1 m3 at a density of 100 kg/m3 slurry and the additive based on (H O ) as well as the
2 2
(after drying curing). packaging (15% of the dry slurry packed in paper
bags, 85% of the dry slurry filled into a dual silo
Declared Unit together with the additive); it also includes the
Name Value Unit production of the silo (and the associated machinery
Gross density (dry) 100 kg/m3 for mixing/installation (allocated based on the
Declared unit 1 m3 estimated total turn­over over their service life).
Module A4 includes the transport of the two
components and the silo/machinery to the construction
3.2 System boundary site.
A life cycle assessment type „cradle to gate with
options, with modules C1 – C4, and module D (A1­A3, Module A5 covers the mixing of the two components,
C1­C3, D and additional modules” is calculated. its installation, the landfilling of the installation (waste)
as well as the thermal treatment of the paper bags
used for packaging in a municipal waste incineration
4 Environmental Product Declaration HOLCIM Deutschland – Airium cement­based insulation foam
part. Due to the very limited amount, no exported expected to contribute significantly to the
energy is declared in A5 nor considered in module D. envi­ronmental indicators declared. Thus, it can be
assumed that the total contribution of the neglected
Module B1 includes the carbonation of the processes is not higher than 5 % of the declared
cementitious foam. impact categories.
Module C1: Mechanical deconstruction is assumed, 3.5 Background data
implying the consumption of diesel in a building ecoinvent v3.8 (cut-off) was used as the background
machine and some dust emissions. database. For cement, a tool­generated, self­
declaration in EPD format is used (Holcim
In Module C2, it is assumed that the de­installed Süddeutschland GmbH, 2022); for the additive based
product is transported to an inert material landfill on H O , a producer­specific, aggregated dataset was
2 2
(scenario 1) or to a sorting platform over 50 km for used.
recycling (scenario 2).
3.6 Data quality
Module C3_2: For the 100% recycling scenario The foreground data are based on extensive and
(scenario 2), it is assumed that the deconstructed wall detailed data collection at the production sites of
including the insulation material are sorted in a sorting Solvay (for H O ), Holcim (recipes, self­declaration in
2 2
plant; during this process, the insulation material will EPD format for cement) and HASIT (mixing and
be converted into a homogeneous powder that installation). The foreground data could be fully linked
reaches “end­of­waste”. It can be further used as a with corresponding data sets from the background
filler in cement or mortar production. database ecoinvent v3.8 (cut-off).
The background data were updated in 2021. The
Module C4_1: For the 100% landfilling scenario quality of the foreground and background data can
(scenario 1), it is assumed that the deinstalled product therefore be assessed as very good.
is disposed of in a landfill for inert materials.
3.7 Period under review
Module D_2: For the recycling scenario, a substitution The data collected represents the specification of the
of milled limestone used in the production of cement or product and the production conditions in 2021.
mortar is assumed.
3.8 Allocation
No co­products are generated during the production of
3.3 Estimates and assumptions the two components nor during the mixing on the
No further assumptions and estimates relevant to the construction site.
results had to be made beyond those described in
sections 3 and 4. No processes were modelled as part of the foreground
model that would have required an allocation of multi­
3.4 Cut-off criteria input processes. Background dataset on municipal
The applicable criteria for the exclusion of inputs and waste incineration plants were taken from ecoinvent
outputs are defined in EN 15804, clause 6.3.5, and in without any modification.
the IBU PCR part A (IBU 2021b), respectively.
All data were taken into account that resulted from the Reuse, recycling and recovery (recycling scenario 2)
data collection procedure in the plants of the different are modelled in line with EN 15804 (see clause 5,
project participants (Solvay, HASIT, Holcim France), Module D for details)
including all components of the recipes, energy and
water consumption, waste treatment, transport, main 3.9 Comparability
infrastructure for onsite preparation of the final product Basically, a comparison or an evaluation of EPD data
and its application, etc. is only possible if all the data sets to be compared
With this approach also mass and energy flows below were created according to EN 15804 and the building
1 percent of total mass and energy flows caused by context, respectively the product­specific
the declared products were included in the characteristics of performance, are taken into account.
assessment.
Beyond that, no material or energy flows were Ecoinvent v3.8 (cut­off) was used as the background
neglected that would have been known by the persons database.
re­sponsible for the project and that could have been
4. LCA: Scenarios and additional technical information
Characteristic product properties
Information on biogenic Carbon
Transport from the gate to the site (A4)
Module A4 contains the average transport scenario
Name Value Unit from the production site to the construction site in
Biogenic carbon content in Germany. A default distance of 80 km is assumed in
0 kg C
product accordance with manufacturer’s information.
Biogenic carbon in packaging 0 kg C The transport includes the two components (as
The minimal quantities of biogenic carbon in methyl installed) and the paper bags as packaging to the
ethyl hydroxy­ethyl cellulose (MHEC) as well as in the construction site. In addition, it includes the transport of
small share of paper packaging are disregarded. the silo + machinery (2850 kg) to and from the
5 Environmental Product Declaration HOLCIM Deutschland – Airium cement­based insulation foam
construction site over the default distance as a sorting platform over 50 km with lorries > 32 metric
mentioned above. tons of emission classes EURO6.
C3: For the 100% landfill scenario (scenario 1), no
Name Value Unit
processes are declared within module C3. The
Transport distance 80 km
declared values are thus 0.
as in
Capacity utilisation (including For the 100% recycling scenario (scenario 2), it is
ecoinvent %
empty runs) assumed that the deconstructed wall including the
dataset
insulation material is sorted in a sorting plant; during
this process, the insulation material will be converted
Assembly (A5)
into a powder that can be further used as a filler in
On the construction site, the components are mixed
cement or mortar production.
and water added to produce the insulation foam ready
to be applied. . Once installed, the insulation foam
C4: For the landfilling scenario (scenario 1), it is
dries and gets inert.
assumed that the deinstalled product is disposed of in
Wastage of 3% is assumed, for its production,
a landfill for inert materials.
transport, mixing and disposal in a landfill (transport
This module is not relevant for the 100% recycling
distance: 50 km) are taken into account. The
scenario.
machinery is cleaned with water twice a day.
Name Value Unit
The paper bags including a PE­foil are assumed to be
Collected as mixed construction
transported 50 km with a lorry 16­32 metric ton, 119.9 kg
waste
EURO6 to an incineration plant with an efficiency R1 <
Recycling ­ kg
0.6 (according to the ecoinvent dataset used); due to
Scenario 1: landfilling 119.9 kg
the negligible quantities, the recovered energy is not
Scenario 2: recycling 119.9 kg
declared as exported energy.
(values including carbonates from carbonation during
use phase)
Name Value Unit
Water consumption 0.0266 m3
Reuse, recovery and (or recycling potentials (D),
Electricity consumption 2.22 kWh
relevant scenario information
Other energy carriers ­ MJ
Material loss 3.9 kg This module is not relevant for the landfilling of
Output substances following 3.9 kg inorganic materials (scenario 1); the amount of
waste treatment on site recovered energy from the thermal treatment of
packaging waste is considered negligeable. Module D
Use or application of the installed product (B1) is thus declared to be “zero”.
Carbonation is estimated based on EN 16757,
Sustainability of construction works – Environmental
For the recycling scenario, a substitution of milled
product declarations – Product category rules for
limestone used in the production of cement or mortar is
concrete and concrete elements, annex BB. Given the
assumed.
high porosity of the material, it is assumed that the
potential to carbonate is fully used over the service life
of the product (several decades).
Reference service life
Name Value Unit
Life Span (according to BBSR) > 50 a
End of Life (C1-C4)
Two scenarios are declared:
Scenario 1: 100% landfilling
Scenario 2: 100% recycling via a sorting plant for
mineral construction waste, separate of the pulverized
Airium cement­based insulation material and use as a
filler in cement or mortar production.
C1: Mechanical deconstruction is assumed, implying a
consumption of diesel in a building machine and some
dust emissions. The corresponding data has been
taken from the UVEK­data base (UVEK 2022, to be
published), commonly used for LCA of construction
products in Switzerland.
C2: As a default, it is assumed that the de­installed
product is transported to an inert material landfill or to
6 Environmental Product Declaration HOLCIM Deutschland – Airium cement­based insulation foam
5. LCA: Results
DESCRIPTION OF THE SYSTEM BOUNDARY (X = INCLUDED IN LCA; ND = MODULE OR INDICATOR NOT
DECLARED; MNR = MODULE NOT RELEVANT)
BENEFITS AND
CONSTRUCTI LOADS
PRODUCT STAGE ON PROCESS USE STAGE END OF LIFE STAGE BEYOND THE
STAGE SYSTEM
BOUNDARIES
7 Environmental Product Declaration HOLCIM Deutschland – Airium cement­based insulation foam
lairetam
waR
ylppus tropsnarT
gnirutcafunaM
eht
morf
tropsnarT
etis
eht
ot
etag
ylbmessA esU
ecnanetniaM
riapeR
tnemecalpeR tnemhsibrufeR
ygrene
lanoitarepO esu
retaw
lanoitarepO esu
noitcurtsnoc­eD
noitilomed tropsnarT
gnissecorp
etsaW
lasopsiD ­esueR ­yrevoceR ­gnilcyceR laitnetop
A1 A2 A3 A4 A5 B1 B2 B3 B4 B5 B6 B7 C1 C2 C3 C4 D
X X X X X X ND MNR MNR MNR ND ND X X X X X
RESULTS OF THE LCA - ENVIRONMENTAL IMPACT according to EN 15804+A2: 1 m³ Airium™ cement-
based insulation foam 100 kg/m³
Core Indicator Unit A1-A3 A4 A5 B1 C1 C2 C3/2 C4/1 D/1 D/2
GWP­total [kg CO2­Eq.] 4.07E+1 4.95E+0 6.74E­2 ­1.99E+1 3.96E­1 9.77E­1 8.77E­1 5.09E­1 0.00E+0 ­2.66E+0
GWP­fossil [kg CO2­Eq.] 4.07E+1 4.95E+0 6.74E­2 ­1.99E+1 3.96E­1 9.76E­1 8.77E­1 5.09E­1 0.00E+0 ­2.66E+0
GWP­biogenic [kg CO2­Eq.] 0.00E+0 0.00E+0 0.00E+0 0.00E+0 0.00E+0 0.00E+0 0.00E+0 0.00E+0 0.00E+0 0.00E+0
GWP­luluc [kg CO2­Eq.] 9.02E­3 1.98E­3 2.02E­6 0.00E+0 3.95E­5 3.90E­4 2.31E­4 1.14E­4 0.00E+0 ­3.99E­3
ODP [kg CFC11­Eq.] 2.06E­6 1.15E­6 7.67E­10 0.00E+0 8.46E­8 2.26E­7 1.91E­7 2.52E­7 0.00E+0 ­1.73E­7
AP [mol H+­Eq.] 8.61E­2 1.41E­2 4.06E­5 0.00E+0 4.11E­3 2.77E­3 7.40E­3 4.99E­3 0.00E+0 ­2.18E­2
EP­freshwater [kg P4­Eq.] 1.42E­3 3.53E­5 6.04E­8 0.00E+0 1.31E­6 6.96E­6 5.87E­6 3.24E­6 0.00E+0 ­2.00E­4
EP­marine [kg N­Eq.] 1.04E­2 2.80E­3 1.72E­5 0.00E+0 1.82E­3 5.51E­4 3.05E­3 1.88E­3 0.00E+0 ­4.23E­3
EP­terrestrial [mol N­Eq.] 2.41E­1 3.12E­2 1.91E­4 0.00E+0 2.00E­2 6.14E­3 3.36E­2 2.07E­2 0.00E+0 ­5.46E­2
POCP [kg NMVOC­Eq.] 6.68E­2 1.20E­2 4.92E­5 0.00E+0 5.49E­3 2.36E­3 9.32E­3 5.92E­3 0.00E+0 ­1.32E­2
ADPE [kg Sb­Eq.] 9.27E­5 1.76E­5 1.80E­8 0.00E+0 2.04E­7 3.46E­6 3.11E­6 9.93E­7 0.00E+0 ­1.14E­5
ADPF [MJ] 2.84E+2 7.51E+1 3.57E­2 0.00E+0 5.43E+0 1.48E+1 1.39E+1 1.65E+1 0.00E+0 ­4.40E+1
[m³ world­Eq
WDP 8.27E+0 2.29E­1 1.07E­3 0.00E+0 8.49E­3 4.51E­2 4.39E­2 5.21E­2 0.00E+0 ­5.07E+0
deprived]
GWP = Global warming potential; ODP = Depletion potential of the stratospheric ozone layer; AP = Acidification potential of land and water; EP =
Caption Eutrophication potential; POCP = Formation potential of tropospheric ozone photochemical oxidants; ADPE = Abiotic depletion potential for non­
fossil resources; ADPF = Abiotic depletion potential for fossil resources; WDP = Water (user) deprivation potential
RESULTS OF THE LCA - INDICATORS TO DESCRIBE RESOURCE USE according to EN 15804+A2: 1 m³
Airium™ cement-based insulation foam 100 kg/m³
Indicator Unit A1-A3 A4 A5 B1 C1 C2 C3/2 C4/1 D/1 D/2
PERE [MJ] 1.70E+1 1.06E+0 1.74E­3 0.00E+0 3.01E­2 2.08E­1 1.65E+0 3.26E­1 0.00E+0 ­7.01E+0
PERM [MJ] 0.00E+0 0.00E+0 0.00E+0 0.00E+0 0.00E+0 0.00E+0 0.00E+0 0.00E+0 0.00E+0 0.00E+0
PERT [MJ] 1.70E+1 1.06E+0 1.74E­3 0.00E+0 3.01E­2 2.08E­1 1.65E+0 3.26E­1 0.00E+0 ­7.01E+0
PENRE [MJ] 2.88E+2 7.51E+1 3.58E­2 0.00E+0 5.43E+0 1.48E+1 1.39E+1 1.65E+1 0.00E+0 ­4.43E+1
PENRM [MJ] 0.00E+0 0.00E+0 0.00E+0 0.00E+0 0.00E+0 0.00E+0 0.00E+0 0.00E+0 0.00E+0 0.00E+0
PENRT [MJ] 2.88E+2 7.51E+1 3.58E­2 0.00E+0 5.43E+0 1.48E+1 1.39E+1 1.65E+1 0.00E+0 ­4.43E+1
SM [kg] 0.00E+0 0.00E+0 0.00E+0 0.00E+0 0.00E+0 0.00E+0 0.00E+0 0.00E+0 0.00E+0 1.20E+2
RSF [MJ] 0.00E+0 0.00E+0 0.00E+0 0.00E+0 0.00E+0 0.00E+0 0.00E+0 0.00E+0 0.00E+0 0.00E+0
NRSF [MJ] 0.00E+0 0.00E+0 0.00E+0 0.00E+0 0.00E+0 0.00E+0 0.00E+0 0.00E+0 0.00E+0 0.00E+0
FW [m³] 1.14E­1 6.69E­3 5.52E­6 0.00E+0 3.09E­4 1.32E­3 9.27E­4 6.45E­4 0.00E+0 ­5.53E­3
PERE = Use of renewable primary energy excluding renewable primary energy resources used as raw materials; PERM = Use of
renewable primary energy resources used as raw materials; PERT = Total use of renewable primary energy resources; PENRE = Use of
non­renewable primary energy excluding non­renewable primary energy resources used as raw materials; PENRM = Use of non­
Caption
renewable primary energy resources used as raw materials; PENRT = Total use of non­renewable primary energy resources; SM = Use
of secondary material; RSF = Use of renewable secondary fuels; NRSF = Use of non­renewable secondary fuels; FW = Use of net fresh
water
RESULTS OF THE LCA – WASTE CATEGORIES AND OUTPUT FLOWS according to EN 15804+A2:
1 m³ Airium™ cement-based insulation foam 100 kg/m³
Indicator Unit A1-A3 A4 A5 B1 C1 C2 C3/2 C4/1 D/1 D/2
HWD [kg] 2.94E­4 1.96E­4 1.21E­7 0.00E+0 1.49E­5 3.86E­5 3.41E­5 1.83E­5 0.00E+0 ­2.86E­5
NHWD [kg] 6.63E+0 3.95E+0 3.10E­3 0.00E+0 9.03E­3 7.79E­1 3.78E­1 1.20E+2 0.00E+0 ­2.06E­1
RWD [kg] 1.64E­3 1.09E­3 3.30E­7 0.00E+0 8.07E­5 2.14E­4 2.19E­4 2.38E­4 0.00E+0 ­5.19E­4
CRU [kg] 0.00E+0 0.00E+0 0.00E+0 0.00E+0 0.00E+0 0.00E+0 0.00E+0 0.00E+0 0.00E+0 0.00E+0
MFR [kg] 0.00E+0 0.00E+0 0.00E+0 0.00E+0 0.00E+0 0.00E+0 1.20E+2 0.00E+0 0.00E+0 0.00E+0
MER [kg] 0.00E+0 0.00E+0 0.00E+0 0.00E+0 0.00E+0 0.00E+0 0.00E+0 0.00E+0 0.00E+0 0.00E+0
EEE [MJ] 0.00E+0 0.00E+0 0.00E+0 0.00E+0 0.00E+0 0.00E+0 0.00E+0 0.00E+0 0.00E+0 0.00E+0
EET [MJ] 0.00E+0 0.00E+0 0.00E+0 0.00E+0 0.00E+0 0.00E+0 0.00E+0 0.00E+0 0.00E+0 0.00E+0
HWD = Hazardous waste disposed; NHWD = Non­hazardous waste disposed; RWD = Radioactive waste disposed; CRU = Components
Caption for re­use; MFR = Materials for recycling; MER = Materials for energy recovery; EEE = Exported electrical energy; EEE = Exported
thermal energy
RESULTS OF THE LCA – additional impact categories according to EN 15804+A2-optional:
1 m³ Airium™ cement-based insulation foam 100 kg/m³
Indicator Unit A1-A3 A4 A5 B1 C1 C2 C3/2 C4/1 D/1 D/2
[Disease
PM 1.19E­6 3.13E­7 2.97E­10 0.00E+0 5.84E­7 6.17E­8 6.46E­7 1.08E­7 0.00E+0 ­1.82E­7
Incidence]
[kBq U235­
IRP 1.05E+2 3.26E­1 1.26E­4 0.00E+0 2.31E­2 6.43E­2 9.25E­2 7.07E­2 0.00E+0 ­3.15E­1
Eq.]
ETP­fw [CTUe] 1.37E+3 5.89E+1 2.02E­1 0.00E+0 3.18E+0 1.16E+1 9.45E+0 9.12E+0 0.00E+0 ­3.06E+2
HTP­c [CTUh] 3.20E­8 1.90E­9 2.64E­11 0.00E+0 1.23E­10 3.74E­10 4.34E­10 2.08E­10 0.00E+0 ­1.35E­9
HTP­nc [CTUh] 1.23E­6 5.96E­8 2.27E­10 0.00E+0 2.30E­9 1.17E­8 9.05E­9 4.32E­9 0.00E+0 ­3.31E­8
SQP [­] 1.47E+2 5.23E+1 1.49E­2 0.00E+0 6.91E­1 1.03E+1 7.49E+0 3.66E+1 0.00E+0 ­1.32E+1
PM = Potential incidence of disease due to PM emissions; IR = Potential Human exposure efficiency relative to U235; ETP­fw = Potential
Caption comparative Toxic Unit for ecosystems; HTP­c = Potential comparative Toxic Unit for humans (cancerogenic); HTP­nc = Potential
comparative Toxic Unit for humans (not cancerogenic); SQP = Potential soil quality index
Disclaimer 1 – for the indicator “Potential Human exposure efficiency relative to U235”.
This impact category deals mainly with the eventual impact of low dose ionizing
radiation on human health of the nuclear fuel cycle. It does not consider effects due to possible
nuclear accidents, occupational exposure nor due to radioactive waste disposal in underground
facilities. Potential ionizing radiation from the soil, from radon and from some construction materials is also not
measured by this indicator.
Disclaimer 2 – for the indicators “abiotic depletion potential for non­fossil resources”, “abiotic depletion potential
for fossil resources”, “water (user) deprivation potential, deprivation­weighted water consumption”, “potential
comparative toxic unit for ecosystems”, “potential comparative toxic unit for humans – cancerogenic”, “Potential
comparative toxic unit for humans ­ not cancerogenic”, “potential soil quality index”.
The results of this environmental impact indicator shall be used with care as the
uncertainties on these results are high or as there is limited experienced with the indicator.
6. LCA: Interpretation
The following Figure illustrates the relative also from transport to the construction site (module
contributions of the different modules along the life A5). Carbonation recaptures around 40 % of the GWP
cycle of the declared products. caused during production (modules A1­A3).
The largest part of environmental impacts – usually Benefits and burdens beyond the system boundary
more than 50% of total impacts ­ is caused during (module D) are in the order of 10 % to 25 % of the
production (modules A1­A3). Comparably high impacts impacts over the product life cycle (modules A1­A3).
– between 10 % and 20 % of total impacts – results
The use of renewable primary energy is mainly caused product – in the recycling scenario this amount is
by the share of renewable energy in the electricity mix, reduced significantly; hazardous and radioactive waste
thus the production stage is the main drivers of this are mainly caused by the electricity mix used in the
impact category; the same holds also for the use of production phase.
non­renewable primary energy. Material use of primary
energy is negligible. As mentioned before, Airium™ insulation foam can
Non­hazardous waste as the quantitatively most also be applied as a 2­layered system with a dry
relevant waste flows is related to the landfilling of the density of 250 kg/m3. While the composition of the two
8 Environmental Product Declaration HOLCIM Deutschland – Airium cement­based insulation foam
densities differs slightly, the values per kg are density of 100 kg/m3. This is considered reasonably
comparably close. The values for Airium™ insulation close for scaling the values from a dry density of 100
foam at a dry density of 250 kg/m3 vary between 81 % kg/m3 to a dry density of 250 kg.
(for Eutrophication, marine) and 112 % (APDe) of the
declared values for Airium™ insulation foam at a dry
7. Requisite evidence
No specific test results are required by the PCR part B.
8. References
Product category rules of IBU
EN 12667
IBU (2021a) DIN EN 12667:2001­05, Thermal performance of
IBU (2021): General Instructions for the EPD building materials and products ­ Determination of
Programme of the Institut Bauen & Umwelt e.V. thermal resistance by means of guarded hot plate and
(General Instructions for the IBU EPD Programme). heat flow meter methods ­ Products of high and
Version 2.0, Institut Bauen & Umwelt, Berlin. medium thermal resistance; German version
EN 12667:2001.
IBU (2021b)
IBU (2021): PCR Part A: Calculation rules for the life EN 10456
cycle assessment and requirements for the project DIN EN ISO 10456:2010­05, Building materials and
report according to EN 15804+A2:2019. Version 2.1., products ­ Hygrothermal properties ­ Tabulated design
Institut Bauen & Umwelt, Berlin. values and procedures for determining declared and
design thermal values (ISO 10456:2007 +
IBU (2020) Cor. 1:2009); German version EN ISO 10456:2007 +
IBU (2020): PCR Part B: Requirements on the EPD for AC:2009.
cement­based foams. Version 2020/05, Institut Bauen
& Umwelt, Berlin. ISO 12572
DIN EN ISO 12572:2017­05, Hygrothermal
performance of building materials and products ­
Standards and legal documents Determination of water vapour transmission
properties ­ Cup method (ISO 12572:2016); German
EN 15804 version EN ISO 12572:2016.
EN 15804+A2:2019+AC:2021, Sustainability of
construction works ­ Environmental product EN 13501
declarations ­ Core rules for the product category EN 13501­1:2018, Fire classification of construction
construction products. products and building elements ­ Part 1: Classification
using data from reaction to fire tests
EN 16757
EN 16757:2017, Sustainability of construction works – EN 998-1
Environmental product declarations – Product category DIN EN 998­1:2017­02, Specification for mortar for
rules for concrete and concrete elements. masonry ­ Part 1: Rendering and plastering mortar;
German version EN 998­1:2016.
ISO 14025
ISO 14025:2006­07, Environmental labels and COUNCIL REGULATION (EU) No 333/2011
declarations ­ Type III Environmental declarations ­ COUNCIL REGULATION (EU) No 333/2011 of 31
Principles and procedures. March 2011 establishing criteria determining when
certain types of scrap metal cease to be waste under
ISO 14044 Directive 2008/98/EC of the European Parliament and
EN ISO 14044:2006­07, Environmental management ­ of the Council.
Life cycle assessment ­ Requirements and guidance
(ISO 14044:2006); German and English versions ECHA cadidate list
EN ISO 14044:2006. The Candidate List of substances of very high concern,
available via https://echa.europa.eu/nl/­/four­
ISO 15686 newsubstances­added­to­the­candidate­list.
ISO 15686, Service life planning (various parts)
Regulation on biocidal products
EN 1602 REGULATION (EU) No 528/2012 OF THE
DIN EN 1602:2013­05, Thermal insulating products for EUROPEAN PARLIAMENT AND OF THE COUNCIL
building applications ­ Determination of the apparent of 22 May 2012 concerning the making available on
density; German version EN 1602:2013. the market and use of biocidal products.
EN 1604 Regulation (EU) Nr. 305/2011(CPR)
DIN EN 1604:2013­05, Thermal insulating products for REGULATION (EU) No 305/2011 OF THE
building applications ­ Determination of dimensional EUROPEAN PARLIAMENT AND OF THE COUNCIL
stability under specified temperature and humidity of 9 March 2011 laying down harmonised conditions
conditions; German version EN 1604:2013.
9 Environmental Product Declaration HOLCIM Deutschland – Airium cement­based insulation foam
for the marketing of construction products and
repealing Council Directive 89/106/EEC. Friedrich & Stocker (2019)
Friedrich K. und Stocker R. (2019): Untersuchung der
COUNCIL REGULATION (EU) No 333/2011 Recyclingfähigkeit und des End­of­Life­Verhaltens des
COUNCIL REGULATION (EU) No 333/2011 of 31 neuen Dämmstoffproduktes „Airium. Studie im Auftrag
March 2011 establishing criteria determining when der Lafarge Zementwerke GmbH, Wien, Version 2,
certain types of scrap metal cease to be waste under Lehrstuhl für Abfallverwertungstechnik und
Directive 2008/98/EC of the European Parliament and Abfallwirtschaft, Leoben (A).
of the Council.
Holcim Süddeutschland GmbH (2022)
European Waste Index Holcim Süddeutschland GmbH (2022): Environmental
http://www.gesetze­im­internet.de/avv/anlage.html data sheet / self­declaration basd on Environdec c­
PCR ­001 Cement and building limes (EN 16908):
Holcim Optimo 5 % Dotternhausen; date of issue:
Additional references 2022­01­25.
BBSR 2017 Stemmler K. (2018)
Bundesinstitut für Bau­, Stadt­ Stemmler K. (2018): Expulsion Tests on a on Wastes
und Raumforschung Service Life of Building from Airium Foam Concrete. Internal project report
Components; version 24.02.2017. P.82007.183, Lafarge Holcim, Mannersdorf (A).
https://www.nachhaltigesbauen.de/fileadmin/pdf/Nutzu
ngsdauer_Bauteile/BNB_Nutzungsdauern_von_Bauteil Weidema et al. (2013)
en_2017­02­24.pdf Weidema, B., C. Bauer, R. Hischier, C. Mutel, T.
Nemecek, J. Reinhard, C.O. Vadenbo, G. Wernet
ecoinvent v3.8 (2013): Overview and methodology, Data quality
ecoinvent v3.8, Ökobilanzdatenbank, 12/2021. guideline for the ecoinvent database version 3.
ecoinvent, Zürich. ecoinvent report no. 1 (v3), St. Gallen (CH).0
10 Environmental Product Declaration HOLCIM Deutschland – Airium cement­based insulation foam
Publisher
Institut Bauen und Umwelt e.V. Tel +49 (0)30 3087748­ 0
Hegelplatz 1 Fax +49 (0)30 3087748­ 29
10117 Berlin Mail info@ibu­epd.com
Germany Web www.ibu-epd.com
Programme holder
Institut Bauen und Umwelt e.V. Tel +49 (0)30 ­ 3087748­ 0
Hegelplatz 1 Fax +49 (0)30 – 3087748 ­ 29
10117 Berlin Mail info@ibu­epd.com
Germany Web www.ibu-epd.com
Author of the Life Cycle
Assessment Tel + 41 (0)44 241 39 06
Dr. Frank Werner ­ Umwelt & Fax + 41 (0)44 461 33 28
Entwicklung Mail frank@frankwerner.ch
Kammelenbergstrasse 30 Web http://www.frankwerner.ch/
9011 St. Gallen
Switzerland
Owner of the Declaration
Holcim (Deutschland) GmbH Tel +49 (0)5132 927 432
Willy­Brand­Straße 69 Fax +49 (0)5132 927 430
20457 Hamburg Mail technisches­
Germany marketing@lafargeholcim.com
Web www.holcim.de
