ENVIRONMENTAL PRODUCT DECLARATION
as per ISO 14025 and EN 15804+A2
Owner of the Declaration Rubner Holding AG - S.p.A.
Publisher Institut Bauen und Umwelt e.V. (IBU)
Programme holder Institut Bauen und Umwelt e.V. (IBU)
Declaration number EPD-HOL-20230236-IBC1-EN
Issue date 28.06.2023
Valid to 27.06.2028
holzius – solid wood slab elements
holzius GmbH - S.r.l.
www.ibu-epd.com | https://epd-online.com
1. General Information
holzius GmbH - S.r.l. holzius – solid wood slab elements
Programme holder Owner of the declaration
IBU – Institut Bauen und Umwelt e.V. Rubner Holding AG - S.p.A.
Hegelplatz 1 Handwerkerzone 2
10117 Berlin 39030 Kiens
Germany Italy
Declaration number Declared product / declared unit
EPD-HOL-20230236-IBC1-EN 1 m³ of HOLZIUS solid wood slab elements with an average density of
495 kg/m³
This declaration is based on the product category rules: Scope:
Solid wood products, 01.08.2021 This EPD is based on a declared unit of 1 m³ of solid wood slab element
(PCR checked and approved by the SVR) (moisture of 13 % at a raw density of 495 kg/m³) produced by HOLZIUS in
Prad/Eyrs (Italy).
Issue date The owner of the declaration shall be liable for the underlying information
and evidence; the IBU shall not be liable with respect to manufacturer
28.06.2023
information, life cycle assessment data and evidences.
The EPD was created according to the specifications of EN 15804+A2. In
Valid to
the following, the standard will be simplified as EN 15804.
27.06.2028
Verification
The standard EN 15804 serves as the core PCR
Independent verification of the declaration and data according to ISO
14025:2011
internally X externally
Dipl.-Ing. Hans Peters
(Chairman of Institut Bauen und Umwelt e.V.)
Florian Pronold Matthias Schulz,
(Managing Director Institut Bauen und Umwelt e.V.) (Independent verifier)
1 Environmental Product Declaration - holzius GmbH - S.r.l. - holzius – solid wood slab elements
2. Product
Constructional data
2.1 Product description/Product definition
HOLZIUS solid wood slab elements (HOLZIUS-SWE) are used Name Value Unit
as solid wood walls, solid wood ceilings and solid wood roofs, Wood types by trade names acc.
spruce, pine, larch -
especially in ecological solid wood construction and for single- to EN 1912
family houses as well as for complex multi-story buildings. Wood moisture acc. to EN
< 17 %
HOLZIUS-SWE, are produced as multilayer solid wood 13183-2
elements based on vertically oriented block elements (squared
Use of wood preservatives (the Where other
timber), free from glue and metal. The single layers of the
wood preservative test mark to preservative means -
HOLZIUS-SWE consist of solid wood planks vertically aligned
DIN 68800-3 must be indicated) are insufficient
and are connected in the plane by tongue and groove. The
Bending strength acc. to EN 338 24 N/mm2
single layers are connected by dovetail-shaped wooden
connectors. Due to the vertical arrangement HOLZIUS Compressive strength parallel 21 N/mm2
elements are free from settling. acc. to EN 338
HOLZIUS solid wood ceiling and roof elements are made of Compressive strength
2.5 N/mm2
parallel arranged squared timber, which interlock by tongue and rectangular acc. to EN 338
groove and are connected by wooden screws in plane. Tensile strength parallel acc. to
The tongue-and-groove connection within HOLZIUS-SWE gives EN 338
14.5 N/mm2
it airtightness without the need for additional foils.
Tensile strength rectangular acc.
Exactly dimensioned free spaces between the squared timber 0.4 N/mm2
to EN 338
components within the single layers of the HOLZIUS-SWE
Modulus of elasticity acc. to EN
allows dimensional stability, independent from changes in 11000 N/mm2
338
humidity.
HOLZIUS solid wood elements are made of softwood according Shear strength acc. to EN 338 4 N/mm2
to EN 1912. For the placing on the market of the products in the Shear modulus acc. to EN 338 690 N/mm2
European Union/European Free Trade Association (EU/EFTA)
depending on
(with the exception of Switzerland) Regulation (EU) No. Dimensional deviation acc. to
geometrical mm
305/2011 /PCR applies. The product needs a Declaration of ETA-15/729 and ETA-17/745/
dimensions
Performance taking into consideration ETA-15/729 holzius
Length < 13.50 m
Vollholzwand, holzius Rippendecke/ and ETA-17/745 holzius
Vollholzelemente and the CE-marking. Width < 3.5 m
For use, the respective national provisions apply. depending on
Height (min. - max.) m
statical requirements
2.2 Application
Gross density acc. to EN 338 420 kg/m3
HOLZIUS-SWE are mainly used as structural components for
Surface quality n.r. -
timber buildings.
Risk class acc. to DIN 68800-3 4 -
2.3 Technical Data Specific heat capacity acc. to EN
1.6 kJ/kgK
The performance data of the products are in accordance with 12664
the Declaration of Performance with respect to its essential Thermal conductivity acc. to EN
characteristics according to ETA-15/729 and ETA-17/745. 12664 0.11 W/(mK)
HOLZIUS-SWE are produced in accordance with ETA-15/729
Calculation value for thermal
and ETA-17/745 with different strength classes. For the n.r. W/(mK)
conductivity
strength class C24 the following applies:
Water vapor diffusion equivalent
air layer thickness acc. to ISO n.r. m
12572
Water vapour diffusion
resistance factor acc. to ISO 20 - 50 -
12572
Formaldehyde emissions acc. to
n.r. μg/m3
EN 717-1
HOLZIUS-SWE are manufactured in accordance with ETA-
15/729 and ETA-17/745 from coniferous species, with
priority being given to spruce, fir, pine and larch. Other
coniferous species are permissible but not typical. HOLZIUS-
SWE are produced from kiln-dried coniferous wood with an
average wood moisture content of around 13 % at delivery.
The mechanical characteristics of HOLZIUS-SWE are in
accordance with strength classes specified in ETA-15/729 and
ETA-17/745. For the determination of the technical
specifications, the declarations of performance (DOP) in the
currently valid versions apply. The dimensional tolerances are
in accordance with ETA-15/729 and ETA-17/745.
The products are manufactured in domestic visual quality,
visual quality or industrial quality. Use of preventive
chemical wood preservatives in accordance with DIN 68800-3
2 Environmental Product Declaration - holzius GmbH - S.r.l. - holzius – solid wood slab elements
is unusual and permitted only if other preservative measures
given in DIN 68800-2 are not sufficient on their own. 2.8 Product processing/Installation
HOLZIUS-SWE can be processed with commercially available
2.4 Delivery status tools. The instructions for occupational safety/assembly are to
HOLZIUS-SWE are produced with the dimensions according to be observed.
chapter 2.3 and is delivered in domestic visual quality, visual
quality or industrial quality. The tolerances according to ETA- 2.9 Packaging
15/729 and ETA-17/745 are met. To protect HOLZIUS-SWE against climatic influences,
polyethylene foils are used in small quantities during
2.5 Base materials/Ancillary materials transportation.
HOLZIUS-SWE comprises kiln-dried coniferous squared timber
according to hEN 14081. Hardwood is used in small quantities 2.10 Condition of use
for the production of fasteners. The composition of HOLZIUS-SWE corresponds to the
composition according to Section 2.5 for the entire period of
HOLZIUS-SWE contains the following proportions of use.
ingredients per m³ on average:
2.11 Environment and health during use
• Coniferous wood (atro), mainly spruce approx. 88-90%
Environmental protection: According to current knowledge, the
• Water approx. 10-12 %
intended use of HOLZIUS-SWE does not present any hazards
• admixture: 0 %
or impairments to water, air and soil.
Health protection: Under normal conditions of use, HOLZIUS-
The products have an average density of 495 kg/m³.
SWE is not expected to cause any damage or impairments to
health.
This product/article/at least one partial article contains
HOLZIUS-SWE subsequently releases formaldehyde during life
substances listed in the candidate list (date: 17.01.2023)
cycle.
exceeding 0.1 percentage by mass: no.
HOLZIUS-SWE have formaldehyde emission values in the
range of the untreated raw material wood (sawn timber,
This product/article/at least one partial article contains other
0.004 ml/m³, Meyer, 1994).
carcinogenic, mutagenic, reprotoxic (CMR) substances in
Due to the product composition, no pollutants that could later
categories 1A or 1B which are not on the candidate list,
be emitted are introduced into the product.
exceeding 0.1 percentage by mass: no.
2.12 Reference service life
Biocide products were added to this construction product or it Solid wood has been used in structural timber construction for
has been treated with biocide products (this then concerns a 100 years. When used as designated, no end of durability must
treated product as defined by the (EU) Ordinance on Biocide be expected due to its natural durability (protection against
Products No. 528/2012): no. moisture). When used as designated, the lifetime of HOLZIUS-
SWE is equal to the duration of use of the building.
2.6 Manufacture
HOLZIUS-SWE are manufactured from sustainable sawn 2.13 Extraordinary effects
timber (PEFC) sourcing from sustainable forestry. Wet sawn Fire
timber is kiln-dried to a moisture content of about 13 % and HOLZIUS-SWE are classified in accordance with ETA-15/729
subsequently pre-planed. To ensure the characteristic values of and ETA-17/745 as follows:
the HOLZIUS-SWE, all individual squared timbers are visually
Fire protection
graded according to EN 14081-1. Weak parts of planks, which
reduce the strength and stiffness properties due to the natural Name Value
growth characteristics of wood, are cut out depending on the Building material class D
grading class. The graded squared timbers are subsequently Burning droplets d0
cut to the required length for further production.
Smoke gas development s2
Subsequently, the required dovetail connections are milled as
well as the screw holes are made in order to assemble the
individual components into final HOLZIUS-SWE afterwards. Water
If necessary, the blanks are cut to their final complex shapes as No ingredients are washed out which could be hazardous to
well as the surfaces are finished. To ensure the product quality, water.
a treatment with weathering or wood preservatives may be
required for transport to the construction site, storage, and Mechanical destruction
during assembly. The fracture behaviour of HOLZIUS-SWE is appearance typical
for solid wood.
2.7 Environment and health during manufacturing
During production, there are no negative impacts on water and 2.14 Re-use phase
soil. The resulting process wastewater is fed into the local In the event of selective de-construction, HOLZIUS-SWE can
sewage system and cleaned according to legal regulations. The easily be re-used after the end of the structure's service life.
resulting exhaust air is cleaned according to the legal The preferred use of HOLZIUS-SWE is in the form of reuse
regulations. based on the applicable country-specific requirements.
Noise emissions from industrial plants are reduced by structural If it is not re-used, it will be subjected to thermal utilization for
measures and comply with the legal requirements. the production of heat and electricity due to the high calorific
The manufacturing process applies to all production facilities value of approx. 16.5 MJ/kg (at a humidity of u = 12 %) in
covered by this EPD. compliance with the applicable country-specific
The employee protection in the manufacturing process requirements.
complies with the respective country-specific requirements,
employees are provided with personal protective equipment.
3 Environmental Product Declaration - holzius GmbH - S.r.l. - holzius – solid wood slab elements
HOLZIUS-SWE are assigned to waste code 17 02 01 in the
2.15 Disposal European list of waste 2014/955/EU.
If the residues are not used for any other cascading use, waste
wood is disposed according to the applicable country-specific 2.16 Further information
requirements. Disposal represents a possible but unusual case. More detailed information is available at: www.holzius.com
3. LCA: Calculation rules
Module C4 | Disposal
3.1 Declared Unit The applied scenario declares the energetic recovery of the
This EPD refers to a declared unit of 1 m³ of solid wood slab wooden products, therefore no environmental impacts are to be
element produced by HOLZIUS. The declared unit refers to an expected from waste processing of the products in C4.
average density of 495 kg/m³ and wood moisture at delivery of
13 %. Module D | Benefits and loads beyond the system
Declared unit boundary
Applying an European average scenario, module D describes
Name Value Unit
the energetic recovery of the product at the end of life including
Declared unit 1 m3 the corresponding energy substitution potentials.
Gross density 495 kg/m3
Wood moisture at delivery 13 %
3.3 Estimates and assumptions
The analysed products represent an average of HOLZIUS solid All assumptions are verified through detailed documentation
wood slab elements produced at Prad (IT). and correspond to the best possible representation of reality
based on the available data. Background data for wood logs
The declared unit was calculated on a volume-weighted basis. refer to generic data for spruce logs in bark derived from the
This EPD refers to an average product manufactured at one GaBi database. Spruce represents the majority of wood
site. All products undergo the same processing steps. A processed at HOLZIUS. The used dataset represents an
possible variability is only expected due to the use of different approximation for all other species.
wood species. The upstream chain for spruce is considered Regional applicability of the used background data refers to
representative. The robustness of the declared LCA values can average data under European or German conditions taken from
thus be classified as high. the GaBi database. German data were used for the Italian
market whenever European or regionalised average data were
3.2 System boundary
not available.
The life cycle assessment of average solid wood slab elements
produced by HOLZIUS refers to a cradle-to-gate analysis of the
Emissions from wood drying were included in the calculations
environmental impacts with modules C1–C4 and module D
according to Rüter & Diederichs 2012.
(A1–A3 + C + D). The following life cycle phases are part of the
analysis: 3.4 Cut-off criteria
The LCA model covers all available input and output flows,
Module A1–A3 | Production stage which can be represented based on robust data and from which
The production stage includes upstream burdens of raw a significant contribution can be expected. Data gaps are filled
materials (mainly fresh and dry lumber) and the corresponding with conservative assumptions of average data or generic data
transports to the production site in Prad (Italy). Direct emissions if available and are documented accordingly.
from the drying of lumber are included in the study and Only data with a contribution of less than 1 % were cut off.
estimated using a worst-case approximation. Thermal energy is Thus, no data were neglected, of which a substantial impact is
delivered from district heating at Prad. The electricity delivered to be expected. All relevant data were collected
stems from a regional supplier, who is using hydropower for its comprehensively. Cutoff material and energy flows were
generation. Due to a lack of electricity certificates, the LCA chosen carefully based on their expected quantitative
results are calculated based on the Italian residual mix. contribution as well as potential environmental impacts. Thus, it
can be assumed that the sum of all neglected input flows does
Module C1 | Deconstruction and demolition not account for more than 5 % of the total material, water and
After the removal of building components overlying the product, energy flows. Environmental impacts of machines, plant and
the joints can simply be loosened by screwing or sawing and infrastructure were not included.
lifted by cranes to the place of removal. Required energy
demand can be neglected. The actual energy demand depends 3.5 Background data
on the installation of the products and can therefore vary This study uses generic background data for the evaluation of
greatly in the building context. upstream environmental impacts from GaBi database 2022.2
as well as recognised literature such as Rüter & Diederichs
Module C2 | Transport to disposal 2012.
Module C2 includes the transport to waste treatment. In this
case, transport by truck over a transport distance of 50 km is 3.6 Data quality
assumed. Data collection is based on product-specific questionnaires. It
follows an iterative process of clarifying questions via e-mail,
Module C3 | Waste processing telephone calls or in personal/web meetings. Intensive
In Module C3, the chipping after the removal of the products is discussions between the RUBNER group and Daxner & Merl
considered. The wooden products and with them the material- result in an accurate mapping of product-related material and
inherent properties leave the product system as secondary energy flows. This leads to a high quality of foreground data
combustibles in module C3. collected. Data collection relies on a consistent process
according to ISO 14044.
4 Environmental Product Declaration - holzius GmbH - S.r.l. - holzius – solid wood slab elements
The technological, geographical and time-related manufactured, used or handled at the end of the product´s
representativeness of the database was kept in mind when lifespan: Italy
selecting background data. Whenever specific data were
missing, either generic datasets or representative average data
3.9 Allocation
were used instead. The implemented GaBi background
datasets refer to the latest versions available and are carefully The carbon content and primary energy content of the products
chosen. were assessed based on their material inherent properties
according to underlying physical relationships.
The assessment of the robustness of the average can be found
3.10 Comparability
in Section 3.1.
Basically, a comparison or an evaluation of EPD data is only
3.7 Period under review possible if all the data sets to be compared were created
Foreground data were collected in the 2021 production year, according to EN 15804 and the building context, respectively
and the data are based on the volumes produced on an annual the product-specific characteristics of performance, are taken
basis. into account.
3.8 Geographic Representativeness The GaBi background database was used to calculate the LCA
Land or region, in which the declared product system is (GaBi 10; 2022.2).
4. LCA: Scenarios and additional technical information
End of life (C1-C4)
Characteristic product properties of biogenic carbon
During tree growth, the wood assimilates carbon dioxide and Name Value Unit
stores biogenic carbon. The carbon stored in the product is Energy recovery 495 kg
declared in the following table.
Reuse, recovery and/or recycling potentials (D), relevant
Information on describing the biogenic Carbon Content at
scenario information
factory gate
Name Value Unit
Name Value Unit
Processing rate 100 %
Biogenic carbon content in product 219 kg C
Efficiency of power plant 68 %
The product reaches the end-of-waste status after removal from
the building, transport to processing and chipping of the
product. For the end of life of the solid wood slab elements,
Installation into the building (A5) energy recovery as secondary fuel in a biomass power plant is
The end of life of the product packaging is not declared in assumed. As the main sales market for solid wood products is
module A5. concentrated in the European region, plant-specific
Name Value Unit characteristic values correspond to a European average
scenario (EU). The scenario considers a reprocessing rate of
Packaging (polyethylene) 0.490 kg
100 % for solid wood products after removal from the building.
The end-of-life scenario used in this LCA study is based on the This assumption has to be adjusted accordingly when applying
following assumptions: the results in the building context. At the end of life of the
product, the equilibrium moisture is comparable to the moisture
content at delivery. This value can vary depending on the
storage of the product before energy recovery.
5 Environmental Product Declaration - holzius GmbH - S.r.l. - holzius – solid wood slab elements
5. LCA: Results
The following table contains the LCA results for a declared unit of 1 m³ of solid wood slab element produced by HOLZIUS (495 kg/m³).
DESCRIPTION OF THE SYSTEM BOUNDARY (X = INCLUDED IN LCA; ND = MODULE OR INDICATOR NOT DECLARED; MNR =
MODULE NOT RELEVANT)
Benefits and
Construction loads beyond
Product stage Use stage End-of-life stage
process stage the system
boundaries
la ire ta m w a Ry lp p u s tro p s n a rT g n iru tc a fu n a M e h t m o rf tro p s n a rTe tis e h t o t e ta g y lb m e s s A e s U e c n a n e tn ia M ria p e R tn e m e c a lp e R tn e m h s ib ru fe R y g re n e la n o ita re p Oe s u re ta w la n o ita re p Oe s u n o itc u rts n o c -e Dn o itilo m e d tro p s n a rT g n is s e c o rp e ts a W la s o p s iD -e s u e R-y re v o c e R-g n ilc y c e Rla itn e to p
A1 A2 A3 A4 A5 B1 B2 B3 B4 B5 B6 B7 C1 C2 C3 C4 D
X X X MND MND MND MND MNR MNR MNR MND MND X X X X X
RESULTS OF THE LCA - ENVIRONMENTAL IMPACT according to EN 15804+A2: 1 m³ HOLZIUS solid wood slab element (495
kg/m³)
Parameter Unit A1-A3 C1 C2 C3 C4 D
Global Warming Potential total (GWP-total) kg CO 2 eq -6.81E+02 0 1.56E+00 8.14E+02 0 -4.36E+02
Global Warming Potential fossil fuels (GWP-fossil) kg CO 2 eq 1.24E+02 0 1.49E+00 3.65E+00 0 -4.11E+02
Global Warming Potential biogenic (GWP-biogenic) kg CO 2 eq -8.06E+02 0 6.49E-02 8.1E+02 0 -2.44E+01
Global Warming Potential luluc (GWP-luluc) kg CO 2 eq 4.14E-01 0 1E-02 7.72E-04 0 -4.91E-02
Depletion potential of the stratospheric ozone layer (ODP) kg CFC11 eq 8.65E-09 0 1.46E-13 5.34E-11 0 -3.18E-09
Acidification potential of land and water (AP) mol H+ eq 6.63E-01 0 4.97E-03 8.02E-03 0 3.41E-01
Eutrophication potential aquatic freshwater (EP-freshwater) kg P eq 2.11E-03 0 5.31E-06 1.07E-05 0 -6.42E-04
Eutrophication potential aquatic marine (EP-marine) kg N eq 2.86E-01 0 2.27E-03 1.8E-03 0 7.38E-02
Eutrophication potential terrestrial (EP-terrestrial) mol N eq 2.92E+00 0 2.54E-02 1.89E-02 0 8.75E-01
Formation potential of tropospheric ozone photochemical oxidants kg NMVOC
7.76E-01 0 4.46E-03 4.86E-03 0 3.13E-01
(POCP) eq
Abiotic depletion potential for non fossil resources (ADPE) kg Sb eq 2.66E-05 0 1.5E-07 9.95E-07 0 -6.83E-05
Abiotic depletion potential for fossil resources (ADPF) MJ 1.62E+03 0 1.95E+01 6.63E+01 0 -7.11E+03
m3 world eq
Water use (WDP) 1.75E+01 0 1.66E-02 8.33E-01 0 -2.34E+01
deprived
RESULTS OF THE LCA - INDICATORS TO DESCRIBE RESOURCE USE according to EN 15804+A2: 1 m³ HOLZIUS solid wood
slab element (495 kg/m³)
Parameter Unit A1-A3 C1 C2 C3 C4 D
Renewable primary energy as energy carrier (PERE) MJ 1.88E+03 0 1.35E+00 8.14E+03 0 -2.19E+03
Renewable primary energy resources as material utilization
MJ 8.1E+03 0 0 -8.1E+03 0 0
(PERM)
Total use of renewable primary energy resources (PERT) MJ 9.98E+03 0 1.35E+00 3.68E+01 0 -2.19E+03
Non renewable primary energy as energy carrier (PENRE) MJ 1.6E+03 0 1.96E+01 6.63E+01 0 -7.11E+03
Non renewable primary energy as material utilization (PENRM) MJ 2.12E+01 0 0 0 0 0
Total use of non renewable primary energy resources (PENRT) MJ 1.62E+03 0 1.96E+01 6.63E+01 0 -7.11E+03
Use of secondary material (SM) kg 0 0 0 0 0 0
Use of renewable secondary fuels (RSF) MJ 0 0 0 0 0 8.1E+03
Use of non renewable secondary fuels (NRSF) MJ 0 0 0 0 0 0
Use of net fresh water (FW) m3 6.73E-01 0 1.56E-03 3.51E-02 0 -1.49E+00
RESULTS OF THE LCA – WASTE CATEGORIES AND OUTPUT FLOWS according to EN 15804+A2:
1 m³ HOLZIUS solid wood slab element (495 kg/m³)
Parameter Unit A1-A3 C1 C2 C3 C4 D
Hazardous waste disposed (HWD) kg 5.29E-06 0 1.04E-10 5.73E-09 0 -8.81E-07
Non hazardous waste disposed (NHWD) kg 2.09E+00 0 3.19E-03 4.99E-02 0 2.46E-01
Radioactive waste disposed (RWD) kg 4.66E-02 0 3.63E-05 1.06E-02 0 -6.3E-01
Components for re-use (CRU) kg 0 0 0 0 0 0
Materials for recycling (MFR) kg 0 0 0 0 0 0
Materials for energy recovery (MER) kg 0 0 0 4.95E+02 0 0
Exported electrical energy (EEE) MJ 0 0 0 0 0 0
Exported thermal energy (EET) MJ 0 0 0 0 0 0
RESULTS OF THE LCA – additional impact categories according to EN 15804+A2-optional:
1 m³ HOLZIUS solid wood slab element (495 kg/m³)
Parameter Unit A1-A3 C1 C2 C3 C4 D
Incidence of disease due to PM emissions (PM) Disease ND ND ND ND ND ND
6 Environmental Product Declaration - holzius GmbH - S.r.l. - holzius – solid wood slab elements
incidence
Human exposure efficiency relative to U235 (IR) kBq U235 eq ND ND ND ND ND ND
Comparative toxic unit for ecosystems (ETP-fw) CTUe ND ND ND ND ND ND
Comparative toxic unit for humans (carcinogenic) (HTP-c) CTUh ND ND ND ND ND ND
Comparative toxic unit for humans (noncarcinogenic) (HTP-nc) CTUh ND ND ND ND ND ND
Soil quality index (SQP) SQP ND ND ND ND ND ND
The additional and optional impact categories according to EN 15804+A2 are not declared, as the uncertainty of these indicators is to
be classified as high.
Disclaimer 1 – for the indicator 'Potential Human exposure efficiency relative to U235'.
This impact category deals mainly with the eventual impact of low-dose ionizing radiation on human health of the nuclear fuel cycle. It
does not consider effects due to possible nuclear accidents, occupational exposure or radioactive waste disposal in underground
facilities. Potential ionizing radiation from the soil, from radon and from some construction materials is also not measured by this
indicator.
Disclaimer 2 – for the indicators 'abiotic depletion potential for non-fossil resources', 'abiotic depletion potential for fossil resources',
'water (user) deprivation potential, deprivation-weighted water consumption', 'potential comparative toxic unit for ecosystems', 'potential
comparative toxic unit for humans – cancerogenic', 'Potential comparative toxic unit for humans - not cancerogenic', 'potential soil
quality index'.
The results of this environmental impact indicator shall be used with care as the uncertainties on these results are high as there is
limited experience with the indicator.
6. LCA: Interpretation
The following interpretation contains a summary of the LCA After its use in the building, the product is assumed to be
results referenced to a declared unit of 1 m³ of HOLZIUS solid incinerated in a biomass power plant. As a result, the
wood slab elements. incorporated carbon is emitted again to the atmosphere
representing biogenic carbon dioxide emissions (module C3).
The global warming potential (GWP) of HOLZIUS products
shows negative values in the production phase (modules A1– The negative values in the end-of-life (module D) result from
A3). These negative impacts result from the use of wood as raw the energetic treatment of the product. As the energy produced
material. Wood sequesters biogenic carbon during tree growth. at the biomass power plant can substitute (mainly fossil) fuels,
The sequestered carbon does not contribute to global warming an environmental net benefit is generated.
as long as it is stored in the biomass.
In the environmental profile of HOLZIUS solid wood elements, and the production process in Prad (Italian residual mix) is a
the supply chain of dry-purchased sawn timber is a driving key driver in addition to the supply chain for dry purchased
force. In terms of the contribution to global warming (GWP) and sawn timber.
the use of fossil resources, the electricity required for drying
7 Environmental Product Declaration - holzius GmbH - S.r.l. - holzius – solid wood slab elements
The results of the previous EPD (EPD-RUB-20180062-IBB1- version due to the update of the underlying methodology
EN) are not directly comparable with the present updated according to EN 15804+A2.
7. Requisite evidence
The following evidence of environmental and health relevance composition for a representative cross-section.
was provided.
7.4 VOC emissions
7.1 Formaldehyde For the verification of VOC emissions, a test report (No. 51005-
Not relevant, as no adhesives containing formaldehyde are 002 III B, 2016) of an emission analysis of pure timber
used in the production process. A test report (No. according to AgBB-Scheme 2015 is available. Analysis was
2117078/CT/2022/1/A1, 2022) confirms a formaldehyde performed in accordance with ISO 16000-3 and ISO 16000-6.
emission below the technical detection limit.
VOC emissions
Name Value Unit
7.2 MDI
No MDI-containing substances are added to the product during Overview of Results (28 days) - μg/m3
production. TVOC (C6 - C16) acc. to AgBB 2015 10 μg/m3
Sum SVOC (C16 - C22) acc. to AgBB 2015 < 5 μg/m3
7.3 Fire gas toxicity
R (dimensionless) acc. to AgBB 2015 0.086 -
Due to the heterogeneous structure of HOLZIUS-SWE,
combined with the non-applicability of the test standard DIN VOC without NIK acc. to AgBB 2015 <5 μg/m3
53436, no relevant measurement results are available, the test Carcinogenic Substances <1 μg/m3
specimen geometry is not able to represent the real gas
8. References
Standards ETA-17/745
ETA-17/745:26.03.2018: holzius Vollholzelemente.
DIN 53436
DIN 53436:2015, Generation of thermal decomposition hEN 14081
products from materials for their analytic-toxicological testing. hEN 14081-1:2016-06-01, Timber structures - Strength graded
structural timber with rectangular cross section - Part 1:
DIN 68800-2 General requirements.
DIN 68800-2:2012-02, Wood preservation – Part 2: Preventive
constructional measures in buildings. ISO 12572
EN ISO 12572:2016, Hygrothermal performance of building
DIN 68800-3 materials and products - Determination of water vapour
DIN 68800-3:2012-02, Wood preservation – Part 3: Preventive transmission properties - Cup method.
protection of wood with wood preservatives.
ISO 14025
EN 338 DIN EN ISO 14025:2011-10, Environmental labels and
DIN EN 338:2016-07, Structural timber - Strength classes. declarations Type III environmental declarations Principles and
procedures.
EN 717-1
DIN EN 717-1:2005-01, Wood-based panels – Determination of ISO 14044
Formaldehyde release – Part 1: Formaldehyde emission by the DIN EN ISO 14044:2006-10, Environmental management - Life
chamber method. cycle assessment - Requirements and guidelines.
EN 1912 ISO 16000-3
EN 1912:2013-10-15, Structural timber - Strength classes - ISO 16000-3:2011, Indoor air - Part 3: Determination of
Assignment of visual grades and species. formaldehyde and other carbonyl compounds in indoor air and
test chamber air - Active sampling method.
EN 12664
EN 12664:2001, Thermal performance of building materials and ISO 16000-6
products - Determination of thermal resistance by means of ISO 16000-6:2011, Indoor air - Part 6: Determination of volatile
guarded hot plate and heat flow meter methods - Dry and moist organic compounds in indoor and test chamber air by active
products with medium and low thermal resistance. sampling on Tenax TA® sorbent, thermal desorption and gas
chromatography using MS or MS-FID.
EN 13183-2
EN 13183-2:2002, Moisture content of a piece of sawn timber -
Part 2: Estimation by electrical resistance method. Further references
EN 15804 AgBB-Scheme 2015
DIN EN 15804:2012+A2:2019+AC:2021, Sustainability of German Committee for HealthRelated Evaluation of Building
construction works Environmental product declarations Core Products (AgBB): Approach to health assessment of emissions
rules for the product category of construction products. of volatile organic compounds (VOCs and SVOCs) from
building products.
ETA-15/729
ETA-15/729:12.20.2017, holzius Vollholzwand, holzius Candidate List
Rippendecke. List of substances of very high concern considered for approval
8 Environmental Product Declaration - holzius GmbH - S.r.l. - holzius – solid wood slab elements
(status 17.01.2023) according to Article 59 para. 10 of the PCR: Solid wood products
REACH Regulation. European Chemicals Agency. Product category rules for building-related products and
services. Part B: EPD requirements for solid wood products.
GaBi Version v2, Berlin: Institut Bauen und Umwelt e.V., 31.05.2023.
GaBi 10, Software-System and Database for Life Cycle
Engineering. 2022.2. Stuttgart, Echterdingen: Sphera, 1992- PCR 305/2011 (EU)
2022. Available at: https://sphera.com/product-sustainability- REGULATION (EU) No 305/2011 OF THE EUROPEAN
gabi-data-search/ PARLIAMENT AND OF THE COUNCIL of 9 March 2011 laying
down harmonised conditions for the marketing of construction
IBU 2021 products and repealing Council Directive 89/106/EEC.
Institut Bauen und Umwelt e.V.: General Programme
Instructions for the Preparation of EPDs at the Institut Bauen Rüter & Diederichs 2012
und Umwelt e.V. (IBU). Version 2.0, Berlin: Institut Bauen und Ökobilanz-Basisdaten für Bauprodukte aus Holz. Work report
Umwelt e.V., 2021. www.ibuepd.com from the Institut für Holztechnologie und Holzbiologie Nr.
2012/1. Hamburg: Johann Heinrich von Thünen-Institut.
Meyer, 1994
Meyer, B, Boehme, C: 1994, Formaldeyhdabgabe von natürlich 1907/2006/EG
gewachsenem Holz, Holzzentralblatt 122 (Formaldeyhd release VERORDNUNG (EG) Nr. 1907/2006 DES EUROPÄISCHEN
of naturally grown wood), S 1969-1972. PARLAMENTS UND DES RATES vom 18. Dezember 2006 zur
Registrierung, Bewertung, Zulassung undBeschränkung
Ordinance on Biocide Products chemischer Stoffe (REACH).
Regulation (EU) No 528/2012 of the European Parliament and
of the Council of 22 May 2012 concerning the making available 2014/955/EU
on the market and use of biocidal products. 2014/955/EU,COMMISSION DECISION of 18 December 2014
amending Decision 2000/532/EC on the list of waste pursuant
PCR part A to Directive 2008/98/EC of the European Parliament and of the
Product category rules for building-related products and Council.
services. Part A: Calculation Rules for the Life Cycle
Assessment and Requirements on the Project Report according
to EN 15804+A2:2019. Version 1.3. Berlin: Institut Bauen und
Umwelt e.V., 2022.
9 Environmental Product Declaration - holzius GmbH - S.r.l. - holzius – solid wood slab elements
Publisher
Institut Bauen und Umwelt e.V. +49 (0)30 3087748- 0
Hegelplatz 1 info@ibu-epd.com
10117 Berlin www.ibu-epd.com
Germany
Programme holder
Institut Bauen und Umwelt e.V. +49 (0)30 3087748- 0
Hegelplatz 1 info@ibu-epd.com
10117 Berlin www.ibu-epd.com
Germany
Author of the Life Cycle Assessment
Daxner & Merl GmbH +43 676 849477826
Schleifmühlgasse 13/24 office@daxner-merl.com
1040 Wien www.daxner-merl.com
Austria
Owner of the Declaration
Rubner Holding AG - S.p.A. 0039 0474 563 777
Handwerkerzone 2 info@rubner.com
39030 Kiens www.rubner.com
Italy
10 Environmental Product Declaration - holzius GmbH - S.r.l. - holzius – solid wood slab elements
