ENVIRONMENTAL PRODUCT DECLARATION
as per ISO 14025 and EN 15804+A2
Owner of the Declaration DBC, EFCC, FEICA, IVK
Programme holder Institut Bauen und Umwelt e.V. (IBU)
Publisher Institut Bauen und Umwelt e.V. (IBU)
Declaration number EPD-DBC-20220175-IBF1-EN
Issue date 29.08.2022
Valid to 28.08.2027
Products based on epoxy-resin, group 2
DBC - Deutsche Bauchemie e.V.
EFCC - European Federation for Construction Chemicals
FEICA - Association of the European Adhesive and Sealant Industry
IVK - Industrieverband Klebstoffe e.V.
www.ibu-epd.com | https://epd-online.com
Umwelt Produktdeklaration Name des Herstellers – Name des Produkts
1. General Information
DBC - Deutsche Bauchemie e.V. Products based on epoxy-resin, group
EFCC - European Federation for 2
Construction Chemicals
FEICA - Association of the European
Adhesive and Sealant Industry
IVK - Industrieverband Klebstoffe e.V.
Programme holder Owner of the declaration
IBU – Institut Bauen und Umwelt e.V. DBC, Mainzer Landstr. 55, D-60329 Frankfurt a.M.
Hegelplatz 1 EFCC, 172 Boulevard du Triomphe, B-1160 Brussels
10117 Berlin FEICA, Rue Belliard 40, B-1040 Brussels
Germany IVK, Völklingerstr. 4, D-40219 Düsseldorf
Declaration number Declared product / declared unit
EPD-DBC-20220175-IBF1-EN 1 kg product based on epoxy-resin, group 2; density 1
- 2,5 g/cm³
This declaration is based on the product Scope:
category rules: This verified EPD entitles the holder to bear the symbol
Reaction resin products, 01.2019 of the Institut Bauen und Umwelt e.V. It exclusively
(PCR checked and approved by the SVR) applies to products produced in Europe and for a
period of five years from the date of issue. This EPD
may be used by members of DBC, EFCC, FEICA and
Issue date
IVK and their members provided it has been proven
29.08.2022
that the respective product can be represented by this
EPD. For this purpose, a guideline is available at the
Valid to secretariats of the four associations. The members of
28.08.2027 the associations are listed on their respective
websites.
The owner of the declaration shall be liable for the
underlying information and evidence; the IBU shall not
be liable with respect to manufacturer information, life
cycle assessment data and evidences.
The EPD was created according to the specifications
of EN 15804+A2. In the following, the standard will be
simplified as EN 15804.
Verification
The standard EN 15804 serves as the core PCR
Independent verification of the declaration and data
according to ISO 14025:2011
Dipl. Ing. Hans Peters internally x externally
(chairman of Institut Bauen und Umwelt e.V.)
Dr. Alexander Röder Matthias Schulz
(Managing Director Institut Bauen und Umwelt e.V.)) (Independent verifier)
2. Product
2.1 Product description/Product definition For the placing on the market in the European
This EPD comprises reactive products based on epoxy Union/European Free Trade Association (EU/EFTA)
(EP) resin and hardening agent; the Volatile Organic with the exception of Switzerland) products falling
Compound (VOC) content is ≤1 % (VOC definition under Regulation (EU) No 305/2011 (CPR) need a
according to Decopaint Directive). The aqueous Declaration of Performance taking into consideration
systems can be formulated as aqueous dispersions on either the relevant harmonised European standard or
the resin or hardening agent side. They comply with the European Technical Assessment and the CE
multiple, often specific functions in the construction, marking. For the application and use of the products
furnishing and repair of structures. The product the respective national provisions apply.
displaying the highest environmental impacts was used 2.2 Application
as a representative product for calculating the Life Products based on epoxy-resins are used for the
Cycle Assessment results (worst-case approach). following applications:
2 Environmental Product Declaration DBC, EFCC, FEICA, IVK – Products based on epoxy-resin, group 2
- Viscosity (EN ISO 3219)
Module 1: Reactive products for protecting and Further essential characteristics in accordance with the
repairing concrete structures manufacturer's technical documentation/declaration of
Products for increasing the durability of concrete and performance
reinforced concrete structures as well as for new
concrete and for maintenance and repair work Module 2: Liquid-applied roof waterproofing kits
(requirements 1.1), products used to restore and/or to The minimum requirements of EAD 030350-00-
replace defective concrete and to protect reinforce- 0402 'Liquid-applied roof waterproofing kits' must be
ment, necessary to extend the service life of a maintained. The essential characteristics are to be
concrete structure exhibiting deterioration (require- specified in accordance with the European technical
ments 1.2), products for structural bonding of assessment (ETA, specification no.).
strengthening materials to an existing concrete
structure (requirements 1.3) and products for concrete Module 3: Reactive products for liquid-applied
injection for filling cracks, voids and interstices in bridge deck waterproofing kits
concrete (requirements 1.4) The minimum requirements of ETAG 033 'Liquid-
applied bridge deck waterproofing kits' must be
Module 2: Liquid-applied roof waterproofing kits maintained. The essential characteristics are to be
Reactive products for waterproofing roof constructions specified in accordance with the European technical
which are applied on site assessment (ETA, specification no.).
Module 3: Reactive products for liquid-applied Module 4: Reactive products for watertight
bridge deck waterproofing kits covering kits
Products for liquid-applied waterproofing for use on The minimum requirements of EAD 030352-00-
concrete bridge decks 0503 'Liquid applied watertight covering kits for wet
room floors and/or walls' must be maintained. The
Module 4: Reactive products for watertight essential characteristics are to be specified in
covering kits accordance with the European Technical Assessment
Products for waterproofing floors and/or walls in wet (ETA, specification no.).
rooms inside buildings
Module 5: Reactive products for liquid-applied
Module 5: Reactive products for liquid-applied waterproofings
waterproofings The minimum requirements of the 'Test principles
Liquid applied products for waterproofing of buildings regarding the issuing of general building authority
inspection test certificates for liquid applied products
Module 6: Screed material, floor screeds and for waterproofing of buildings' (PG-FLK) must be
decorative floors maintained. The characteristics for the proof of
Products for screed/synthetic resin screed and usability are to be specified in accordance with the
decorative floors for use in floor constructions 'Test principles for granting general building authority
test certificates for liquid applied polymer products for
Module 7: Reactive products for waterproofing waterproofing buildings'.
and/or for pre-treating mineral substrates
Products to protect mineral substrates from the ingress Module 6: Screed material, floor screeds and
of water decorative floors
The requirements on essential characteristics
2.3 Technical Data according to EN 13813 'Screed material and floor
The density of the products is between 1,0 and 2,5 screeds – Screed materials – Properties and
g/cm³, other relevant technical data can be found in the requirements' must be maintained. For synthetic resin
manufacturer’s technical documentation. screeds, these are:
- Bond strength (EN 13892-8)
Module 1: Reactive products for protecting and - Reaction to fire (EN 13501-1)
repairing concrete structures Further essential characteristics in accordance with the
1.1 The requirements on essential characteristics for manufacturer's technical documentation/declaration of
all intended uses in accordance with EN 1504-2, performance
Tables 1 and 5 must be maintained. These are:
- Permeability to CO (EN 1062-6) Module 7: Reactive products for waterproofing
2
- Water vapour permeability (EN ISO 7783-1/-2) and/or for pre-treating mineral substrates
- Capillary absorption and permeability to water (EN Essential characteristics in accordance with the
1062-3) manufacturer's technical documentation
- Adhesive strength by pull-off test (EN 1542)
1.2 The requirements on essential characteristics for
all intended uses in accordance with EN 1504-3,
Tables 1 and 3, must be maintained. These are
- Compressive strength (EN 12190)
- Chloride content (EN 1015-17)
- Adhesive strength by pull-off test (EN 1542) 2.4 Delivery status
1.3 Essential characteristics for all intended uses in Liquid or pasty in containers made of tinplate or plastic
accordance with EN 1504-4, Tables 3.1 and 3.2 packed in separate or combi-containers for the
(manufacturer's declaration of performance) required mixing ratio. Packages containing one kg of
1.4 Requirements on essential characteristics for all product in different types of containers. Sealants in
intended uses in accordance with EN 1504-5, Table 3: plastic cartridges and foil packs. Typical container
- Injectability (EN 1771) sizes contain 10 to 25 kg of material. For major works,
3 Environmental Product Declaration DBC, EFCC, FEICA, IVK – Products based on epoxy-resin, group 2
vats containing approx. 200 kg or IBCs containing 2.6 Manufacture
more than 1 tonne are also used. The LCA is based on The components of the formulation are usually mixed
a sheet steel container. batch-wise and packaged for delivery.
2.5 Base materials/Ancillary materials 2.7 Environment and health during
The products based on epoxy-resin, comprise glycidyl manufacturing
components (epoxy resin and/or diluting agents) and a As a general rule, no other environmental protection
crosslinking agent component. When installed on site measures other than those specified by law are
hardening occurs with the crosslinking agent necessary.
component. For this purpose, polyamines, polyamides,
polyamine adducts or mixtures of the same are used. 2.8 Product processing/Installation
Additionally the formulation can contain auxiliaries The products based on epoxy-resin are processed by
such as accelerators, catalysts, wetting agents, foam trowelling/knife-coating or rolling, pouring, spraying or
regulators and viscosity regulators for fine adjustment injection. Precautions for safe handling and storage
of the product properties. The mixing ratio for the (e.g. air exchange, exhaust ventilation, personal
glycidyl components and the crosslinker is adjusted in protective measures, precautions required in the
accordance with the stoichiometric requirements. handling of isocyanates and conditions for safe
Product crosslinking starts immediately after mixing the storage) must be observed in accordance with the
components. Typically, the products covered by this information on the safety data sheet.
EPD contain the following range of base materials and The products based on epoxy-resin react after mixing
auxiliaries: resin and crosslinking agent under heat generation
Resin component: ~ 0-90 % (exothermicity). The mixed components must therefore
Reactive diluting agent: ~ 0-90 % be processed swiftly within the pot life indicated. If
Crosslinker component: ~ 5-25 % larger volumes of the mixture remain in the container,
Filler: ~ 0-70 % this can lead to overheating and decomposition. In the
Water: ~ 0-40 % case of reactively diluted products, exothermicity is
Other: <4 % particularly strong. Emissions of volatile components
VOC: ≤1 % according to Decopaint may occur.
Directive (mandatory)
2.9 Packaging
These ranges are average values and the composition A detailed description of packaging is provided in
of products complying with the EPD can deviate from section 2.4. Empty containers and clean foils can be
these concentration levels in individual cases. More recycled.
detailed information is available in the respective
manufacturer's documentation (e.g. product data
sheets). 2.10 Condition of use
Note: For companies to declare their products within During the use phase, products based on epoxy-resin
the scope of this EPD it is not sufficient to simply are crosslinked and essentially comprise an inert
comply with the product composition shown above. three-dimensional network. They are long-lasting
The application of this EPD is only possible for products which protect our buildings in the form of
member companies of DBC, EFCC, FEICA, and IVK adhesives, coatings or sealants as well as make an
member associations and only for specific formulations essential contribution towards retaining their function
with a total score below the declared maximum score and long-term value.
for a product group according to the associated
guidance document. 2.11 Environment and health during use
1. substances from the “Candidate List of Option 1: Products for applications outside indoor
Substances of Very High Concern for areas with permanent stays by people
Authorisation” (SVHC) During use, the reactive products lose their reactive
If this product contains substances listed in the properties and become inert. No risks are known for
candidate list (latest version) exceeding 0.1 water, air and soil if the products are used as
percentage by mass, the relevant information can be designated.
found in the safety data sheet of the relevant product Option 2 :Products for applications inside indoor
covered by this model EPD. areas with permanent stays by people
2. CMR substances in categories 1A and 1B When used in indoor areas with permanent stays by
If this product contains other carcinogenic, mutagenic, people, evidence of the emission performance of
reprotoxic (CMR) substances in categories 1A or 1B construction products in contact with indoor air must be
which are not on the candidate list, exceeding 0.1 submitted according to national requirements (see
percentage by mass, the relevant information can be chapter 7). No further influences by emissions on the
found in the safety data sheet of the relevant product environment and health are known.
covered by this model EPD.
3. Biocide products added to the construction 2.12 Reference service life
product Cured reactive epoxy products comply with a variety
If this construction product contains biocide products, of, often specific, functions in the construction or
the active substances, information on the refurbishment of building structures. They decisively
concentration and/or concentration range, the product improve the usability of building structures and
type together with information on their hazardous significantly extend their original service lives. The
properties are listed in the safety data sheet of the anticipated reference service life depends on the
respective product. specific installation situation and the exposure
associated with the product. It can be influenced by
weathering as well as mechanical or chemical loads.
4 Environmental Product Declaration DBC, EFCC, FEICA, IVK – Products based on epoxy-resin, group 2
linked products. If the crosslinked products can be
2.13 Extraordinary effects removed from construction products without large
effort, thermal recovery is a practical recycling variant
Fire on account of their energy content. Minor adhesion is
Even without any special fire safety features, cured not taken into consideration during disposal. It does
reactive epoxy products comply with at least the not interfere with the disposal/recycling of the
requirements of EN 13501-1 standard for fire classes E remaining components/building materials.
and Efl. In terms of the volumes applied, they only
have a marginal influence on the fire performance 2.15 Disposal
characteristics (e.g. smoke gas development) of the Residual material which cannot be used or recycled
building structure in which they are installed. As must be combined at a specified ratio and hardened.
crosslinked epoxy products are duroplastic they do not Hardened product residue is not special waste. Non-
melt or drip and they do not contribute to the spreading hardened product residue is special waste. Empty,
of fire, whereas the combustibility of crosslinked epoxy dried containers (free of drops and scraped clean) are
products is larger than that of other duroplastics. directed to the recycling process. Residue must be
Among other substances, formaldehyde and phenol directed to proper waste disposal taking into
can be formed in the event of a fire. consideration the local guidelines. The following waste
codes according to the European List of Waste
Water (2000/532/EC) can apply:
Cured reactive epoxy products are chemically inert and Hardened product residue:
insoluble in water. They are often used to protect European Waste Catalogue (EWC) code 08 01 12
building structures from harmful water ingress or the (Paint and varnish waste with the exception of that
effects of flooding. covered by EWC 08 01 11)
EWC code 08 04 10 (Adhesive and sealant compound
Mechanical destruction waste with the exception of that covered by EWC 08
Mechanical destruction of cured reactive epoxy 04 09)
products does not lead to any decomposition products
which are harmful to the environment or health. 2.16 Further information
More information is available on the manufacturer's
2.14 Re-use phase product or safety data sheets and on the
According to present knowledge, no environmentally manufacturer's websites or on request. Valuable
harmful effects are generally anticipated in landfilling, technical information is also available on the
for example, as a result of de-construction and associations' websites.
recycling of building materials with adherent cross-
3. LCA: Calculation rules
3.1 Declared Unit - A4 Transport to site
This EPD refers to the declared unit of 1 kg of product - A5 Installation, product applied into the building
based on epoxy-resin, group 2; applied into the during A5 phase operations and packaging disposal.
building with a density of 1 - 2.50 g/cm³ in accordance The end of life for the packaging material considered is
with the IBU PCR part B for reaction resin products. described below:
The results of the Life Cycle Assessment provided in -Incineration, for materials like wood.
this declaration have been selected from the product -Landfill, for inert material like metals (where used).
with the highest environmental impact (worst-case -C1-C2-C3-D
scenario). The building deconstruction (demolition process) takes
Depending on the application, a corresponding place in the C1 module which considers energy
conversion factor such as the density to convert production and consumption in terms of diesel and all
volumetric use to mass must be taken into the emissions connected with the fuel-burning process
consideration. to run the machines. After the demolition, the product
is transported to the end-of-life processing (C2
The Declaration type is according to EN 15804: Cradle module) where all the impacts related to the transport
to gate with options, modules C1–C4, and module D processes are considered. For precautionary principle
(A1–A3, C, D) and additional modules (A4-A5) and as a worst-case scenario, thermal treatment is the
only end-of-life scenario considered. This is modelled
Declared unit by the incineration process (module C3) where the
Name Value Unit product ends its life cycle.
Declared unit 1 kg Module D accounts for potential benefits that are
Gross density 1 - 2.50 g/cm^3 beyond the defined system boundaries. Credits are
generated during the incineration of wastes and related
electricity produced that are occurring in the A5
module.
3.2 System boundary
Modules A1, A2 and A3 are taken into consideration in 3.3 Estimates and assumptions
the LCA: For this EPD formulation and production data defined
- A1 Production of preliminary products and collected by FEICA were considered. Production
- A2 Transport to the plant waste was assumed to be disposed of by incineration
- A3 Production incl. provision of energy, production of without credits as a worst case.
packaging as well as auxiliaries and consumables and An average of steel and wooden pallets was
waste treatment considered in the LCA
5 Environmental Product Declaration DBC, EFCC, FEICA, IVK – Products based on epoxy-resin, group 2
Production data and packaging are based on details
3.4 Cut-off criteria provided by the manufacturer. The formulation used for
All raw materials submitted for the formulations and evaluation refers to a specific product.
production data were taken into consideration. The data quality of the background data is considered
The manufacture of machinery, plant and other to be good.
infrastructure required for the production of the
products under review was not taken into consideration 3.7 Period under review
in the LCA. Representative formulations are valid for 2021.
Transport of packaging materials is excluded.
3.8 Allocation
3.5 Background data Mass allocation has been applied when primary data
Data from the GaBi database SP40 (2020) was used have been used and implemented into the LCA model.
as background data.
3.9 Comparability
3.6 Data quality Basically, a comparison or an evaluation of EPD data
Representative products were applied for this EPD and is only possible if all the data sets to be compared
the product in the group displaying the highest were created according to EN 15804 and the building
environmental impact was selected for calculating the context, respectively the product-specific
LCA results. The background data sets used are less characteristics of performance, are taken into account.
than 4 years old.
The GaBi database SP40 (2020) was used.
4. LCA: Scenarios and additional technical information
Characteristic product properties
Information on biogenic Carbon
The packaging material contains biogenic carbon
content which is presented below.
Information on describing the biogenic Carbon
Content at factory gate
Name Value Unit
Biogenic Carbon Content in
0 kg C
product
Biogenic Carbon Content in
0.026 kg C
accompanying packaging
For the preparation of building life cycle assessments,
it must be taken into account that in module A5
(installation in the building) the biogenic amount of CO
2
(0.026 kg C *3.67 = 0.095 kg CO -eq.) of the
2
packaging bound in module A1-A3 is mathematically
booked out.
Transport to the building site (A4)
Name Value Unit
Transport distance 1000 km
Gross weight 34 - 40 t
Payload capacity 27 t
Installation into the building (A5)
Name Value Unit
Other resources for packaging
0.117 kg
material
Material loss 0.01 kg
Material loss regards the amount of product not used
during the application phase into the building. This
amount is 1 % of the product, impacts related to the
production of this part are charged to A5 module. This
percentage is considered as waste to disposal and
impacts of its end of life have been considered into the
LCA model and declared in the A5.
End of life (C1-C4)
Name Value Unit
Collected as mixed construction
1 kg
waste
Incineration 1 kg
6 Environmental Product Declaration DBC, EFCC, FEICA, IVK – Products based on epoxy-resin, group 2
5. LCA: Results
DESCRIPTION OF THE SYSTEM BOUNDARY (X = INCLUDED IN LCA; ND = MODULE OR INDICATOR NOT
DECLARED; MNR = MODULE NOT RELEVANT)
BENEFITS AND
CONSTRUCTI LOADS
PRODUCT STAGE ON PROCESS USE STAGE END OF LIFE STAGE BEYOND THE
STAGE SYSTEM
BOUNDARIES
7 Environmental Product Declaration DBC, EFCC, FEICA, IVK – Products based on epoxy-resin, group 2
lairetam
waR
ylppus tropsnarT
gnirutcafunaM
eht
morf
tropsnarT
etis
eht
ot
etag
ylbmessA esU
ecnanetniaM
riapeR
tnemecalpeR tnemhsibrufeR
ygrene
lanoitarepO esu
retaw
lanoitarepO esu
noitcurtsnoc-eD
noitilomed tropsnarT
gnissecorp
etsaW
lasopsiD -esueR -yrevoceR -gnilcyceR laitnetop
A1 A2 A3 A4 A5 B1 B2 B3 B4 B5 B6 B7 C1 C2 C3 C4 D
X X X X X ND ND MNR MNR MNR ND ND X X X ND X
RESULTS OF THE LCA - ENVIRONMENTAL IMPACT according to EN 15804+A2: 1 kg of product based on
epoxy-resin, group 2
Core Indicator Unit A1-A3 A4 A5 C1 C2 C3 D
GWP-total [kg CO2-Eq.] 1.06E+1 5.35E-2 2.49E-1 2.79E-4 1.24E-2 9.45E-1 -3.80E-1
GWP-fossil [kg CO2-Eq.] 1.06E+1 5.30E-2 1.15E-1 2.66E-4 1.18E-2 4.29E-1 -3.79E-1
GWP-biogenic [kg CO2-Eq.] -3.34E-2 1.55E-4 1.34E-1 1.24E-5 5.42E-4 5.15E-1 -8.54E-4
GWP-luluc [kg CO2-Eq.] 5.07E-3 4.29E-4 5.45E-5 6.39E-9 2.79E-7 3.50E-5 -2.38E-4
ODP [kg CFC11-Eq.] 4.95E-14 6.36E-18 5.19E-16 2.84E-20 1.24E-18 3.02E-16 -3.53E-15
AP [mol H+-Eq.] 1.60E-2 1.59E-4 1.91E-4 3.60E-6 3.73E-5 5.25E-4 -5.01E-4
EP-freshwater [kg P-Eq.] 4.73E-5 1.61E-7 4.78E-7 5.75E-11 2.51E-9 1.04E-7 -4.38E-7
EP-marine [kg N-Eq.] 5.25E-3 7.07E-5 6.24E-5 1.63E-6 1.72E-5 2.01E-4 -1.33E-4
EP-terrestrial [mol N-Eq.] 5.45E-2 7.92E-4 6.78E-4 1.79E-5 1.89E-4 2.52E-3 -1.42E-3
POCP [kg NMVOC-Eq.] 1.85E-2 1.40E-4 2.12E-4 4.91E-6 3.39E-5 5.22E-4 -3.83E-4
ADPE [kg Sb-Eq.] 8.97E-6 3.80E-9 9.02E-8 8.06E-12 3.52E-10 4.62E-9 -5.76E-8
ADPF [MJ] 1.83E+2 7.05E-1 1.89E+0 3.81E-3 1.66E-1 5.52E-1 -6.40E+0
[m³ world-Eq
WDP 7.14E-1 4.73E-4 2.22E-2 5.27E-7 2.30E-5 1.57E-1 -3.51E-2
deprived]
GWP = Global warming potential; ODP = Depletion potential of the stratospheric ozone layer; AP = Acidification potential of land and water; EP =
Caption Eutrophication potential; POCP = Formation potential of tropospheric ozone photochemical oxidants; ADPE = Abiotic depletion potential for non-
fossil resources; ADPF = Abiotic depletion potential for fossil resources; WDP = Water (user) deprivation potential
RESULTS OF THE LCA - INDICATORS TO DESCRIBE RESOURCE USE according to EN 15804+A2: 1 kg of
product based on epoxy-resin, group 2
Indicator Unit A1-A3 A4 A5 C1 C2 C3 D
PERE [MJ] 1.51E+1 3.96E-2 1.10E+0 1.20E-5 5.25E-4 9.36E-2 -1.26E+0
PERM [MJ] 9.36E-1 0.00E+0 -9.36E-1 0.00E+0 0.00E+0 0.00E+0 0.00E+0
PERT [MJ] 1.60E+1 3.96E-2 1.69E-1 1.20E-5 5.25E-4 9.36E-2 -1.26E+0
PENRE [MJ] 1.53E+2 7.06E-1 1.90E+0 3.81E-3 1.67E-1 3.06E+1 -6.40E+0
PENRM [MJ] 3.00E+1 0.00E+0 0.00E+0 0.00E+0 0.00E+0 -3.00E+1 0.00E+0
PENRT [MJ] 1.83E+2 7.06E-1 1.90E+0 3.81E-3 1.67E-1 5.52E-1 -6.40E+0
SM [kg] 0.00E+0 0.00E+0 0.00E+0 0.00E+0 0.00E+0 0.00E+0 0.00E+0
RSF [MJ] 0.00E+0 0.00E+0 0.00E+0 0.00E+0 0.00E+0 0.00E+0 0.00E+0
NRSF [MJ] 0.00E+0 0.00E+0 0.00E+0 0.00E+0 0.00E+0 0.00E+0 0.00E+0
FW [m³] 2.65E-2 4.59E-5 6.20E-4 2.16E-8 9.41E-7 3.70E-3 -1.45E-3
PERE = Use of renewable primary energy excluding renewable primary energy resources used as raw materials; PERM = Use of
renewable primary energy resources used as raw materials; PERT = Total use of renewable primary energy resources; PENRE = Use of
non-renewable primary energy excluding non-renewable primary energy resources used as raw materials; PENRM = Use of non-
Caption
renewable primary energy resources used as raw materials; PENRT = Total use of non-renewable primary energy resources; SM = Use
of secondary material; RSF = Use of renewable secondary fuels; NRSF = Use of non-renewable secondary fuels; FW = Use of net fresh
water
RESULTS OF THE LCA – WASTE CATEGORIES AND OUTPUT FLOWS according to EN 15804+A2:
1 kg of product based on epoxy-resin, group 2
Indicator Unit A1-A3 A4 A5 C1 C2 C3 D
HWD [kg] -9.89E-6 3.28E-8 -9.87E-8 3.70E-13 1.62E-11 1.77E-9 -2.54E-9
NHWD [kg] 7.54E-2 1.08E-4 4.86E-2 3.90E-7 1.70E-5 1.36E-1 -2.80E-3
RWD [kg] 4.01E-3 8.73E-7 4.23E-5 4.09E-9 1.79E-7 2.51E-5 -4.28E-4
CRU [kg] 0.00E+0 0.00E+0 0.00E+0 0.00E+0 0.00E+0 0.00E+0 0.00E+0
MFR [kg] 0.00E+0 0.00E+0 0.00E+0 0.00E+0 0.00E+0 0.00E+0 0.00E+0
MER [kg] 0.00E+0 0.00E+0 0.00E+0 0.00E+0 0.00E+0 0.00E+0 0.00E+0
EEE [MJ] 0.00E+0 0.00E+0 2.01E-1 0.00E+0 0.00E+0 0.00E+0 0.00E+0
EET [MJ] 0.00E+0 0.00E+0 3.66E-1 0.00E+0 0.00E+0 0.00E+0 0.00E+0
HWD = Hazardous waste disposed; NHWD = Non-hazardous waste disposed; RWD = Radioactive waste disposed; CRU = Components
Caption for re-use; MFR = Materials for recycling; MER = Materials for energy recovery; EEE = Exported electrical energy; EEE = Exported
thermal energy
RESULTS OF THE LCA – additional impact categories according to EN 15804+A2-optional:
1 kg of product based on epoxy-resin, group 2
Indicator Unit A1-A3 A4 A5 C1 C2 C3 D
[Disease
PM ND ND ND ND ND ND ND
Incidence]
[kBq U235-
IRP ND ND ND ND ND ND ND
Eq.]
ETP-fw [CTUe] ND ND ND ND ND ND ND
HTP-c [CTUh] ND ND ND ND ND ND ND
HTP-nc [CTUh] ND ND ND ND ND ND ND
SQP [-] ND ND ND ND ND ND ND
PM = Potential incidence of disease due to PM emissions; IR = Potential Human exposure efficiency relative to U235; ETP-fw = Potential
Caption comparative Toxic Unit for ecosystems; HTP-c = Potential comparative Toxic Unit for humans (cancerogenic); HTP-nc = Potential
comparative Toxic Unit for humans (not cancerogenic); SQP = Potential soil quality index
Potential Human exposure efficiency relative to U235, Disclaimer 1 – This impact category deals mainly with the
eventual impact of low dose ionizing radiation on human health of the nuclear fuel cycle. It does not consider
effects due to possible nuclear accidents, occupational exposure nor radioactive waste disposal in underground
facilities. Potential ionizing radiation from the soil, radon and (from) some construction materials is also not
measured by this indicator.
ADP minerals & metals, ADP fossil, WDP, ETF-fw, HTP-c, HTP-nc, SQP, Disclaimer 2 – The results of this
environmental impact indicator shall be used with care as the uncertainties on these results are high or as there is
limited experience with the indicator.
Additional environmental impact indicators (suggested by EN15804, table 4) are not declared in the EPD. The
results of this environmental impact indicator shall be used with care as the uncertainties on these results are high
and as there is limited experience with the indicator (see International Reference Life Cycle Data System (ILCD)
classification in EN 15804, table 5). For this reason, results based on these indicators are not considered suitable
for a decision-making process and are thus not declared in the EPD.
6. LCA: Interpretation
The majority of impacts are associated with the renewable energy resources required for the
production phase (A1-A3). The most significant generation and supply of electricity. It should be noted
contribution to the production phase impacts is the that Primary Energy Demand – Renewable (PERT)
upstream production of raw materials as the main generally represents a small percentage of the
driver. Another relevant contributor in the production production phase primary energy demand with the bulk
phase, in the category of Abiotic depletion potential for of the demand coming from non-renewable energy
non-fossil resources (ADPminerals& metals), is the resources.
steel sheet used as a packaging material. Emissions Transportation to the construction site (A4) and the
associated with the manufacturing of products also installation process (A5) make a low contribution to the
have some influence on the Formation potential of overall impacts. Climate change from land use change
tropospheric ozone (POCP) in the production phase. In is the only indicator influenced by transport processes,
all EPDs, CO is the most important contributor to due to the diesel production used as fuel, because part
2
Global Warming Potential (GWP). For the Acidification of this diesel has been produced from bio-based raw
Potential (AP), NOx and SO contribute (to) the largest materials.
2
share. The installation phase mainly influences climate
The majority of life cycle energy consumption takes change indicators, due to the impact related to the
place during the production phase (A1-A3). Significant incineration processes used for packaging waste
contributions to Primary Energy Demand – Non- treatment and residual product treatment (1 % of the
renewable (PENRT) come from the energy re-sources total mass).
used in the production of raw materials. The largest The end-of-life phases influence climate change
contributor to Primary Energy Demand – Renewable indicators, due to the thermal treatment process of the
(PERT) impacts comes from the consumption of resin occurring in C3 module.
7. Requisite evidence
VOC any of the existing regulations or in any of the existing
Special tests and evidence have not been carried out voluntary labelling programs for low-emitting products,
or provided within the framework of drawing up this as far as these
Model EPD. Some member states require special (1) include limits for the parameters TVOC, TSVOC,
documentation on VOC emissions into indoor air for carcinogens, formaldehyde, acetaldehyde, LCI limits
specific areas of application. This documentation, as for individual substances (including but not limited to
well as documentation for voluntary VOC labelling, has the European list of harmonized LCIs), and the R-
to be provided separately and is specific to the product value;
in question. (2) base their test methods on EN 16516;
(3) perform testing and apply the limits after 28 days
Evidence pertaining to VOC emissions shall show of storage in a ventilated test chamber, under the
- either an attestation of compliance with, conditions specified in EN 16516; some regulations
- or documentation of test data that are required in
8 Environmental Product Declaration DBC, EFCC, FEICA, IVK – Products based on epoxy-resin, group 2
and programmes also have limits after 3 days, on top - TSVOC: 100 µg/m³
of the 28 days limits; - Each carcinogen: 1 µg/m³
(4) express the test results as air concentrations in - Formaldehyde: 100 µg/m³
the European Reference Room, as specified in EN - LCI: different per substance involved
16516. - R-value: 1 (meaning that, in total, 100% of the
combined LCI values must not be exceeded).
Examples of such regulations are the Belgian Royal Informative Annexes (2 tables):
Decree C-2014/24239, or the German AgBB/ ABG. Table 1 shown below is an overview of the most
Examples of such voluntary labeling programs are relevant regulations and specifications as of October
EMICODE, Blue Angel or Indoor Air Comfort. 2021, as regards requirements after 3 days of storage
in a ventilated test chamber.
Relevant test results shall be produced either by an Table 2 provides an overview of the most relevant
ISO 17025 accredited commercial test lab or by a regulations and specifications as of October 2021, as
qualified internal test lab of the manufacturer. regards requirements after 28 days of storage in a
Examples of the applied limits after 28 days of storage ventilated test chamber. Some details may be missing
in a ventilated test chamber are: in the table due to lack of space. Values given
- TVOC: 1000 µg/m³ represent maximum values/limits.
8. References
ETAG 033 EN 1015-17:2005-01, Methods of test for mortar for
ETAG 033:2010-09 masonry - Part 17: Determination of water-soluble
Liquid applied bridge deck waterproofing chloride content of fresh mortars
EN 1015-17 EN 1062-3
9 Environmental Product Declaration DBC, EFCC, FEICA, IVK – Products based on epoxy-resin, group 2
EN 1062-3:2008-04, Paints and varnishes - Coating EN 13813:2002-10, Screed material and floor screeds
materials and coating systems for exterior masonry - Screed materials - Properties and requirements
and concrete - Part 3: Determination of liquid water
permeability EN 13892
EN 13892:2003-02, Methods of test for screed
EN 1062-6 materials - Part 8: Determination of bond strength
EN 1062-6:2002-10, Paints and varnishes - Coating
materials and coating systems for exterior masonry ISO 14025
and concrete - Part 6: Determination of carbon dioxide DIN EN ISO 14025:2011-10, Environmental labels and
permeability declarations — Type III environmental declarations —
Principles and procedures
EN 1504-2
EN 1504-2:2004-10, Products and systems for the EN 15804
protection and repair of concrete structures - EN 15804+A2+AC:2021, Sustainability of construction
Definitions, requirements, quality control and works — Environmental Product Declarations — Core
evaluation of conformity - Part 2: Surface protection rules for the product category of construction products
systems for concrete
EN 16516
EN 1504-3 EN 16516:2017
EN 1504-3:2005-12, Products and systems for the Construction products - Assessment of release of
protection and repair of concrete structures - dangerous substances - Determination of emissions
Definitions, requirements, quality control and into indoor air
evaluation of conformity - Part 3: Structural and non-
structural repair EN ISO 17025
EN ISO 17025:2018-03
EN 1504-4 General requirements for the competence of testing
EN 1504-4:2004-11, Products and systems for the and calibration laboratories
protection and repair of concrete structures -
Definitions, requirements, quality control and EAD 030350-00-0402
evaluation of conformity- Part 4: Structural bonding EAD 030350-00-0402:2018-08, Liquid Applied Roof
Waterproofing Kits
EN 1504-5
EN 1504-5:2004-12, Products and systems for the EAD 030352-00-0503
protection and repair of concrete structures - EAD 030352-00-0503:2019-01, Watertight covering
Definitions, requirements, quality control and kits for wet room floors and or walls Part 1: Liquid
evaluation of conformity - Part 5: Concrete injection Applied Coverings with or without wearing surface Part
2: Kits based on flexible sheets Part 3: Kits based on
EN 1542 inherently watertight boards
EN 1542:1999-07, Products and systems for the
protection and repair of concrete structures - Test 2000/532/EC
methods - Measurement of bond strength by pull-off Commission decision dated 3 May 2000 replacing
decision 94/3/EC on a waste directory in accordance
EN 1771 with Article 1 a) of Council Directive 75/442/EEC on
EN 1771:2004-11, Products and systems for the waste and Council decision 94/904/EC on a directory
protection and repair of concrete structures - Test of hazardous waste in terms of Article 1, paragraph 4
methods - Determination of injectability and splitting of Directive 91/689/EEC on hazardous waste
test
Belgian Royal Decree C-2014/24239
EN ISO 3219 Belgisch Staatsblad 8 MEI 2014, p. 60603. —
EN ISO 3219:1994-10, Plastics - Polymers/resins in Koninklijk besluit tot vaststelling van de
the liquid state or as emulsions or dispersions - drempelniveaus voor de emissies naar het
Determination of viscosity using a rotational viscometer binnenmilieu van bouwproducten voor bepaalde
with defined shear rate geoogde gebruiken
EN ISO 7783 Blue Angel
EN ISO 7783-1/-2:2019-02, Paints and varnishes - Environmental label organised by the federal
Determination of water-vapour transmission properties government of Germany www.blauer-engel.de
- Cup method
Candidate list
EN 12190 Candidate List of substances of very high concern for
EN 12190:1998-12, Products and systems for the Authorisation, published in accordance with Article
protection and repair of concrete structures - Test 59(10) of the REACH Regulation, ECHA,
methods - Determination of compressive strength of www.echa.europa.eu/candidate-list-table
repair mortar
CPR
EN 13501-1 CPR Regulation (EU) No 305/2011 of the European
EN 13501-1:2018, Fire classification of construction Parliament and of the Council of 9 March 2011 laying
products and building elements - Part 1: Classification down harmonised conditions for the marketing of
using data from reaction to fire tests construction products and repealing Council Directive
89/106/EEC
EN 13813
10 Environmental Product Declaration DBC, EFCC, FEICA, IVK – Products based on epoxy-resin, group 2
Decopaint Directive www.ibu-epd.com
Directive 2004/42/CE of the European Parliament and
the council of 21 April 2004 on the limitation of Indoor Air Comfort
emissions of volatile organic compounds due to the Product certification by Eurofins, Hamburg, Germany
use of organic solvents in certain paints and varnishes www.eurofins.com
and vehicle refinishing products and amending
Directive 1999/13/EC PCR Part A
Product Category Rules for Building-Related Products
EMICODE and Services, Part A: Calculation Rules for the Life
EMICODE, GEV – Gemeinschaft Cycle Assessment and Requirements on the Project
Emissionskontrollierte Verlegewerkstoffe, Klebstoffe report, Version 1.1, Institut Bauen und Umwelt e.V.,
und Bauprodukte e. V. (pub.).www.emicode.de 2021-01
EWC PCR Part B
2000/532/EC European Waste Catalogue / Ordinance Product Category Rules for Construction Products,
on European List of Wastes Part B: Reaction resin products, 2019-01
European List of Waste PG-FLK
2000/532/EC European Waste Catalogue / Ordinance PG-FLK:2019-07
on European List of Wastes Testing principles regarding the issuing of general
building authority inspection certificates for liquid
GaBi 10 software & documentation applied products for waterproofing of buildings
Data base for Life Cycle Engineering LBP, University
of Stuttgart and Sphera, documentation of GaBi 10 REACH
data sets http://documentation.gabi-software.com/, Directive (EG) No. 1907/2006 of the European
2020 Parliament and of the Council dated 18 December
2006 on the registration, evaluation, approval and
German AgBB restriction of chemical substances (REACH), for
Committee for Health-related Evaluation of Building establishing a European Agency for chemical
Products: health-related evaluation of emissions of substances, for amending Directive 1999/45/EC and
volatile organic compounds (VOC and SVOC) from for annulment of Directive (EEC) No. 793/93 of the
building products; status: June 2012 Council, Directive (EC) No. 1488/94 of the
www.umweltbundesamt.de/produkte/bauprodukte/agb Commission, Guideline 76/769/EEC of the Council and
b.htm Guidelines 91/155/EEC, 93/67/EEC, 93/105/EC and
2000/21/EC of the Commission
IBU 2021
Institut Bauen und Umwelt e.V.: General Instructions
for the EPD programme of Institut Bauen und Umwelt
e.V. EPD programme. Version 2.0. Berlin: Institut
Bauen und Umwelt e.V., 2021
11 Environmental Product Declaration DBC, EFCC, FEICA, IVK – Products based on epoxy-resin, group 2
Publisher
Institut Bauen und Umwelt e.V. Tel +49 (0)30 3087748- 0
Hegelplatz 1 Fax +49 (0)30 3087748- 29
10117 Berlin Mail info@ibu-epd.com
Germany Web www.ibu-epd.com
Programme holder
Institut Bauen und Umwelt e.V. Tel +49 (0)30 - 3087748- 0
Hegelplatz 1 Fax +49 (0)30 – 3087748 - 29
10117 Berlin Mail info@ibu-epd.com
Germany Web www.ibu-epd.com
Author of the Life Cycle
Assessment Tel +49 (0)711 341817-0
Sphera Solutions GmbH Fax +49 (0)711 341817-25
Hauptstraße 111- 113 Mail info@sphera.com
70771 Leinfelden-Echterdingen Web www.sphera.com
Germany
Owner of the Declaration
EFCC - European Federation for Tel +32289720-39
Construction Chemicals Fax +32289720-37
Boulevard du Triomphe 172 Mail info@efcc.be
1160 Brussels Web www.efcc.eu
Belgium
Tel +32 (0)267 673 20
FEICA - Association of the Fax +32 (0)267 673 99
European Adhesive and Sealant Mail info@feica.eu
Industry Web www.feica.eu
Rue Belliard 40 box 10
1040 Brussels
Belgium
Tel +49 (0)69 2556-1318
Fax +49 (0)69 2556-1319
Mail info@deutsche-bauchemie.de
Deutsche Bauchemie e.V. Web www.deutsche-bauchemie.de
Mainzer Landstr. 55
60329 Frankfurt
Germany
Tel +49 (0)211 67931-10
Fax +49 (0)211 67931-33
Mail info@klebstoffe.com
Industrieverband Klebstoffe e.V Web www.klebstoffe.com
Völklinger Straße 4
40219 Düsseldorf
Germany
