ENVIRONMENTAL PRODUCT DECLARATION
as per ISO 14025 and EN 15804+A2
Owner of the Declaration FEICA, EFCC, IVK, DBC
Programme holder Institut Bauen und Umwelt e.V. (IBU)
Publisher Institut Bauen und Umwelt e.V. (IBU)
Declaration number EPD-DBC-20220219-IBF1-EN
Issue date 26.09.2022
Valid to 25.09.2027
Modified mineral mortars, group 3
FEICA - Association of the European Adhesive and Sealant Industry
EFCC - European Federation for Construction Chemicals
IVK - Industrieverband Klebstoffe e.V.
DBC - Deutsche Bauchemie e.V.
www.ibu-epd.com | https://epd-online.com
Umwelt Produktdeklaration Name des Herstellers – Name des Produkts
1. General Information
DBC - Deutsche Bauchemie e.V.
EFCC - European Federation for Modified mineral mortars, group 3
Construction Chemicals
FEICA - Association of the European
Adhesive and Sealant Industry
IVK - Industrieverband Klebstoffe e.V.
Programme holder Owner of the declaration
IBU – Institut Bauen und Umwelt e.V. DBC, Mainzer Landstr. 55, D-60329 Frankfurt a.M.
Hegelplatz 1 EFCC, 172 Boulevard du Triomphe, B-1160 Brussels
10117 Berlin FEICA, Rue Belliard 40, B-1040 Brussels
Germany IVK, Völklingerstr. 4, D-40219 Düsseldorf
Declaration number Declared product / declared unit
EPD-DBC-20220219-IBF1-EN 1 kg of modified mineral mortar with a density 800 -
1,700 kg/m³
This declaration is based on the product Scope:
category rules: This verified EPD entitles the holder to bear the
Mineral factory-made mortar, 11.2017 symbol of the Institut Bauen und Umwelt e.V. It
(PCR checked and approved by the SVR) exclusively applies to products produced in Europe and
for a period of five years from the date of issue. This
EPD may be used by members of FEICA, EFCC, DBC
Issue date
and IVK and their members provided it has been
26.09.2022
proven that the respective product can be represented
by this EPD. For this purpose, a guideline is available
Valid to at the secretariats of the four associations. The
25.09.2027 members of the associations are listed on their
respective websites.
The owner of the declaration shall be liable for the
underlying information and evidence; the IBU shall not
be liable with respect to manufacturer information, life
cycle assessment data and evidences.
The EPD was created according to the specifications
of EN 15804+A2. In the following, the standard will be
simplified as EN 15804.
Verification
The standard EN 15804 serves as the core PCR
Independent verification of the declaration and data
according to ISO 14025:2011
Dipl. Ing. Hans Peters internally x externally
(chairman of Institut Bauen und Umwelt e.V.)
Dr. Alexander Röder Matthias Schulz
(Managing Director Institut Bauen und Umwelt e.V.)) (Independent verifier)
2. Product
2.1 Product description/Product definition For the placing on the market in the European
Modified mineral mortars are combinations of one or Union/European Free Trade Association (EU/EFTA)
more inorganic binders, fillers, aqueous dispersions or with the exception of Switzerland) products falling
dispersion powders, water and if necessary additives. under the Regulation (EU) No 305/2011 (CPR) need a
They comply with manifold, often specific, functions in Declaration of Performance taking into consideration
the construction, furnishing and refurbishment of either the relevant harmonised European standard or
buildings. The product displaying the highest the European Technical Assessment and the CE
environmental impacts was used as a representative marking. For the application and use of the products
product for calculating the Life Cycle Assessment the respective national provisions apply.
results (worst-case approach).
2 Environmental Product Declaration DBC, EFCC, FEICA, IVK – Modified mineral mortar, group 3
2.2 Application Module 1: Modified mineral mortars as repair
Modified mineral mortars are used for the following mortar for the protection and repair of concrete
applications: structures
1.1 Products used to restore and/or replace defective
Module 1: Modified mineral mortars as repair concrete
mortar for the protection and repair of concrete The requirements on essential characteristics for all
structures intended uses in accordance with EN 1504­3, Tables 1
1.1 Products used to restore and/or replace defective and 3, must be maintained. These are:
concrete - Compressive strength (EN 12190)
1.2 Products to protect reinforcement, necessary to - Chloride ion content (EN 1015­17)
extend the service life of a concrete structure exhibiting - Adhesive strength by pull-off test (EN 1542)
deterioration
1.2 Products to protect reinforcement
Module 2: Adhesives based on modified mineral The requirements on essential characteristics for all
mortars intended uses in accordance with EN 1504­7, Table 1,
2.1 Products for bonding ceramic tiles as well as must be maintained. This is
natural stone for internal and external installations on - Corrosion protection (EN 15183)
walls, floors and ceilings Further essential characteristics in accordance with the
2.2 Products for bonding thermal insulation composite manufacturer's technical documentation/declaration of
panels performance
Module 3: Modified mineral mortars as joint fillers Module 2: Adhesives based on modified mineral
Products for joint filling of wall and floor coverings mortars
made of ceramic tiles as well as natural stone for 2.1 Products for bonding ceramic tiles as well as
indoor and outdoor applications natural stone for internal and external installations on
walls, floors and ceilings
Module 4: Modified mineral mortars as screed, The requirements on essential characteristics
floor levelling compounds, fillers, flowing screed according to EN 12004, Table 1, must be maintained.
Products for screed/synthetic resin screed for use in These are:
floor constructions - Tensile adhesion strength after dry storage (EN
12004­2)
Module 5: Modified mineral mortars as levelling - Tensile adhesion strength after water immersion (EN
compounds for walls and ceilings 12004­2)
Products for levelling and repairing rough, uneven - Tensile adhesion strength after heat ageing (EN
walls, for repairing grit spots, closing blowholes and 12004­2)
modelling broken corners and edges - Tensile adhesion strength after freeze/thaw cycles
(EN 12004­2)
Module 6: Modified mineral mortars as grouts - Open time: Tensile strength (EN 12004­2)
Products for grouting on holes, recesses, concrete Further essential characteristics in accordance with the
precast columns, foundations and for anchoring manufacturer's technical documentation/declaration of
machine components indoors and outdoors performance
2.2 The minimum requirement of EAD 040083­00­0404
Module 7: Modified mineral mortars for liquid External Thermal Insulation Composite Systems with
applied products for waterproofing of buildings Rendering must be maintained. The essential
Products for providing cement-based waterproofing characteristics are to be specified in accordance with
surfaces in structural and civil engineering. For use in the European technical assessment (ETA,
new and old buildings as well as beneath tiles specification no.). Further essential characteristics in
7.1 Liquid-applied water impermeable products for use accordance with the manufacturer's technical
beneath ceramic tiling documentation/declaration of performance
7.2 Products for waterproofing with mineral
waterproofing slurries or flexible polymer modified thick Module 3: Modified mineral mortars as joint fillers
coatings The minimum requirements of EN 13888 must be
7.3 Products for water proofing in conjunction with maintained.
ceramic tiles
7.4 Products for waterproofing with flexible polymer Module 4: Modified mineral mortars as screed,
modified mineral thick coatings floor levelling compounds, fillers, flowing screed
The requirements on essential characteristics
Module 8: Modified mineral mortars for according to EN 13813 ‘Screed material and floor
waterproofing floors and/or walls inside buildings screeds – Screed materials – Properties and
Products for watertight covering in wet rooms inside requirements’ must be maintained. For synthetic resin
buildings screeds, these are:
- Bond strength (EN 13892­8)
2.3 Technical Data - Reaction to fire (EN 13501­1)
The density of the products is between 0,80 and 1,70 Further essential characteristics in accordance with the
g/cm³, other relevant technical data can be found in the manufacturer's technical documentation/declaration of
manufacturer’s technical documentation. performance
Construction products with Declaration of Performance
in accordance with CPR and the manufacturer's Module 5: Modified mineral mortars as levelling
technical documentation: compounds for walls and ceilings
Module 5.1: The minimum requirements of EN 998­1
apply. These are: - Reaction to fire (EN 13501­1) -
3 Environmental Product Declaration DBC, EFCC, FEICA, IVK – Modified mineral mortar, group 3
Compressive strength - Dry bulk density - Capillary
water absorption - Water vapour permeability
Further essential characteristics in accordance with the
manufacturer's technical documentation/declaration of
performance 2.4 Delivery status
Module 5.2: The minimum requirements of EN 13279 Modified mineral mortars are generally manufactured
apply. Further essential characteristics in accordance and supplied as factory-made dry mortars. Factory-
with the manufacturer's technical made dry mortar is a finished mixture of base materials
documentation/declaration of performance which merely requires the addition of water and/or a
polymer dispersion on the building site. The products
Module 6: Modified mineral mortars as grouts can be supplied in 1-5 kg bags, 15-25 kg sacks, big
The requirements of DAfStb Guideline on 'Production bags (1 t), minitainers (1.2 t) or as silo goods (5-15 t).
and use of cement-bound flow concrete and grouting Paper sacks with polyethylene lining were modelled as
mortar' (VeBMR) must be maintained. packaging (worst-case approach).
The requirements according to MVV TB No. C 2.1.4.5
for "Ü-mark" must be maintained. 2.5 Base materials/Ancillary materials
Typically, the products covered by this EPD contain
Module 7: Modified mineral mortars for liquid the following range of base materials and auxiliaries
applied products for waterproofing of buildings (% by mass):
7.1 Inorganic binder: ~ 2 - 98
The requirements according to EN 14891 , table 1, Filler materials: ~ 0 - 90
must be maintained. These are: Additives: ~ 0 - 10
- initial tensile adhesion strength EN 14891 Aqueous dispersion and/or dispersion powder: ~ 0 - 35
- Tensile adhesion strength after water contact EN
14891 These ranges are average values and the composition
- Waterproofing EN 14891 of products complying with the EPD can deviate from
- Crack bridging ability EN 14891 these concentration levels in individual cases. More
7.2 detailed information is available in the respective
The minimum requirements of the 'Testing principles manufacturer's documentation (e.g. product data
for granting general building authority approved test sheets).
certificates for waterproofing with mineral Note: For companies to declare their products within
waterproofing slurries and flexible polymer modified the scope of this EPD it is not sufficient to simply
thick coatings' (PG MDS/FPD) must be maintained. comply with the product composition shown above.
The characteristics for the proof of usability are to be The application of this EPD is only possible for
specified in accordance with the test principles for member companies of DBC, EFCC, FEICA, and IVK
granting general building authority test certificates for member associations and only for specific formulations
waterproofing with mineral waterproofing slurries and with a total score below the declared maximum score
flexible polymer thick coatings. for a product group according to the associated
7.3 guidance document.
The minimum requirements of the 'testing principles for
granting general building authority approved test
certificates for waterproofing in conjunction with 1. substances from the “Candidate List of
ceramic tiles' (PG AIV) must be considered. Substances of Very High Concern for
7.4 Authorisation” (SVHC)
The minimum requirement of EAD 030295­00­ If this product contains substances listed in the
0605 must be maintained. The essential characteristics candidate list (latest version) exceeding 0.1
are to be specified in accordance with the European percentage by mass, the relevant information can be
technical assessment (ETA, specification no.). found in the safety data sheet of the relevant product
covered by this model EPD.
Module 8: Modified mineral mortars for 2. CMR substances in categories 1A and 1B
waterproofing floors and/or walls inside buildings If this product contains other carcinogenic, mutagenic,
The minimum requirement of EAD 030352­00­ reprotoxic (CMR) substances in categories 1A or 1B
0503 must be maintained. The essential characteristics which are not on the candidate list, exceeding 0.1
are to be specified in accordance with the European percentage by mass, the relevant information can be
technical assessment (ETA, specification no.). found in the safety data sheet of the relevant product
covered by this model EPD.
3. Biocide products added to the construction
product
Constructional data If this construction product contains biocide products,
Name Value Unit the active substances, information on the
Compressive strength - N/mm2 concentration and/or concentration range, the product
Adhesive shear strength - N/mm2 type together with information on their hazardous
Water absorption - mg properties are listed in the safety data sheet of the
Water vapor diffusion equivalent air respective product.
- m
layer thickness
Thermal conductivity - W/(mK)
Tensile bond strength - N/mm2 2.6 Manufacture
Flexural strength - N/mm2 The raw materials are stored in silos, big bags or sacks
in the manufacturing plant and fed gravimetrically in
Sound absorption coefficient (if
- % accordance with the respective formula and mixed
relevant)
intensively. The mix is then packaged.
4 Environmental Product Declaration DBC, EFCC, FEICA, IVK – Modified mineral mortar, group 3
screed, waterproofing material or repair product,
2.7 Environment and health during makes an essential contribution towards improving
manufacturing building function and value.
The state of the art involves maximum recirculation of
dry waste into production. Wherever dust is incurred 2.11 Environment and health during use
during production in the plant, it is directed to a filter Owing to the stable crystalline bond and firm structure
system considering the limit values applicable for the achieved after curing, emissions are extremely low and
workplace and using the corresponding extraction harmless to health when the respective products are
plants. Sack discharge stations connected to the used in accordance with the designated purpose. No
extraction plant offer employees additional protection risks are known for water, air and soil if the products
from dust. Most of the dust collected in the filter system are used as designated. Natural ionising radiation from
and any residue incurred during production is returned mineral mortar is extremely low and negligible in terms
to the manufacturing process. of health hazards. Options for applications in indoor
Powder residues: Residual product is returned to the areas with permanent stays by people: Evidence of the
production process wherever possible. emission performance of construction products in
Air: Process air is dedusted autonomously, whereby contact with indoor air and depending on the
the values are far below legal requirements. designated use must be submitted for applications in
Water: The production process does not involve water. indoor areas with permanent stays by people, e.g. in
Very low volumes of water are required for laboratory accordance with the German AgBB test scheme or the
tests and for sanitary facilities. GEV (Gemeinschaft Emissionskontrollierte
Noise: Noise level measurements have indicated that Verlegewerkstoffe, Klebstoffe und Bauprodukte e.V.,
all values established within the production facility fall Düsseldorf) EMICODE® marking system typically
below the hearing protection limit of 85dB(A). applied in Germany.
Waste: The main types of waste are powder waste,
paper (paper bags) and foil. Low volumes of metal 2.12 Reference service life
scrap (metal containers), waste oil (maintenance), Modified mineral mortars decisively improve the
wood (pallets) and commercial waste are incurred. All usability of building structures and significantly extend
waste is separated, stored and redirected to the their original service lives. The anticipated reference
recycling circuit or disposed of. service life depends on the specific installation
situation and the exposure associated with the product.
It can be influenced by weathering as well as
2.8 Product processing/Installation mechanical or chemical loads.
Modified mineral mortars can be processed both
automatically and manually. The mortars are either
automatically removed from a silo using a dry conveyor 2.13 Extraordinary effects
or manually taken from the container, mixed with water
and installed. The professional liability association's Fire
rules apply as well as the respective safety data sheets In accordance with Commission Decision 94/611EC,
pertaining to the construction products. On account of modified mineral binding agents comprising finely
the various hydrate levels of cement, lime and calcium distributed organic components must always be
sulphate binding agents in the mineral mortar, the classified in reaction-to-fire class A1 ‘No contribution to
fresh mortar mixed with water is usually strongly fire’ in accordance with EN 13501­1.
alkaline. In the case of more extensive contact, this Where higher percentages of organic components are
alkaline state can cause serious damage to eyes and involved, it can also be assumed that at least the
skin. Therefore, any contact with eyes or skin must be requirements of EN 13501­1 are maintained for fire
avoided by taking personal protective measures, and class E and Efl.
the information outlined on the safety data sheet must
be observed. Uncontrolled dust emissions should be
avoided. Modified mineral mortars may not be Fire protection
discharged into the sewage system, surface water or Name Value
groundwater. Waste incurred on the building site Building material class -
(packaging, pallets, residual mortar) must be collected Burning droplets -
separately. Suitable waste disposal companies Smoke gas development -
dispose of packaging materials and mortar sacks and
return them to the recycling circuit. Dry mortar residue Water
is taken back by the manufacturing plants and used as No relevant volumes of water-soluble substances
a raw material. No dry mortar residue in mortar sacks hazardous to water are washed out when hardened
is incurred. Hard mortar residue can be recycled or modified mineral mortars are exposed to water (e.g.
disposed of as building site rubble. flooding). Modified mineral mortar is stable in terms of
structure and is not subject to any changes in form
2.9 Packaging when exposed to water and drying. If non-hardened
A detailed description of packaging is provided in modified mineral mortars are exposed to water an
section 2.4. Empty, trickle-free paper containers and increase of the pH will take place.
clean PE foils can be recycled.
Mechanical destruction
The mechanical destruction of modified mineral
2.10 Condition of use mortars does not lead to any decomposition products
A modified mineral mortar does not rot and is which are harmful to the environment or health. Dust
resistant to ageing when used in accordance with the incurred during de-construction should be avoided by
designated purpose of the respective products. It is a
durable product which, when used as adhesive,
5 Environmental Product Declaration DBC, EFCC, FEICA, IVK – Modified mineral mortar, group 3
taking the appropriate measures (e.g. humidification). amounts do not play a role when the construction
product is disposed of. They do not interfere with the
disposal/recycling of other components/building
2.14 Re-use phase materials.
Components manufactured using modified mineral The following waste codes according to the European
mortars can usually be easily demolished. When a List of Waste (2000/532/EC) can apply:
building is removed, the materials do not need to be Mineral mortar: EWC 17 01 01 and EWC 10 13 14
treated as special waste; care should, however, be Mineral filler and levelling compound: EWC 17 01 07
taken to ensure unmixed residual materials wherever Calcium sulphate-based filler and levelling compound:
possible. Modified mineral mortars can usually be EWC 17 08 02
redirected to normal building material recycling circuits.
Re-use is generally in the form of recycled aggregate
in building construction and civil engineering. No 2.16 Further information
practical experience is currently available for reusing More information is available on the manufacturer's
components comprising cementitious-based products product or safety data sheets and is available on the
after decommissioning. manufacturer's websites or on request. Valuable
technical information is also available on the
2.15 Disposal associations' websites.
The portion of a modified mineral mortar applied to
another construction product is rather low. These low
3. LCA: Calculation rules
3.1 Declared Unit transported to the end-of-life processing (C2 module)
This EPD refers to the declared unit of 1 kg of modified where all the impacts related to the transport
mineral mortar, group 3; applied into the building with a processes are considered. For precautionary principle
density of 800 - 1,700 kg/m³ in accordance with and as a worst-case scenario, landfilling is the only
the IBU PCR part B for Mineral Factory-Made Mortars. end-of-life scenario considered. This is modelled by
The results of the Life Cycle Assessment provided in the landfill process (module C4) where the product
this declaration have been selected from the product ends its life cycle.
with the highest environmental impact (worst-case Module D accounts for potential benefits that are
scenario). beyond the defined system boundaries. Credits are
Depending on the application, a corresponding generated during the incineration of packaging material
conversion factor such as the density to convert that is occurring in the A5 module.
volumetric use to mass must be taken into
consideration. 3.3 Estimates and assumptions
For this EPD formulation and production data defined
The Declaration type is according to EN 15804: Cradle and collected by FEICA were considered. Production
to gate with options, modules C1–C4, and module D waste was assumed to be disposed of by landfilling as
(A1–A3, C, D) and additional modules (A4-A5). a worst-case.
An average of paper sacks with polyethylene lining and
Declared unit wooden pallets was considered in the LCA.
Name Value Unit
Declared unit 1 kg 3.4 Cut-off criteria
800 - All raw materials submitted for the formulations and
Gross density kg/m3
1700 production data were taken into consideration.
The manufacture of machinery, plant and other
infrastructure required for the production of the
products under review was not taken into consideration
3.2 System boundary in the LCA.
Modules A1, A2 and A3 are taken into consideration in Transport of packaging materials is excluded.
the LCA:
- A1 Production of preliminary products 3.5 Background data
- A2 Transport to the plant Data from the GaBi 10 database SP40 (2020) was
- A3 Production incl. provision of energy, production of used as background data.
packaging as well as auxiliaries and consumables and
waste treatment 3.6 Data quality
- A4 Transport to site Representative products were applied for this EPD and
- A5 Installation, product applied into the building the product in the group displaying the highest
during A5 phase operations and packaging disposal. environmental impact was selected for calculating the
The end of life for the packaging material considered is LCA results. The background datasets used are less
described below: than 4 years old.
-Incineration, for materials like plastic, wood and Production data and packaging are based on details
paper. provided by the manufacturer. The formulation used for
-C1-C2-C4-D evaluation refers to a specific product.
The building deconstruction (demolition process) takes The data quality of the background data is considered
place in the C1 module which considers energy to be good.
generation and consumption of diesel and all the
emissions connected with the fuel-burning process to 3.7 Period under review
run the machines. After the demolition, the product is Representative formulations are valid for 2021.
6 Environmental Product Declaration DBC, EFCC, FEICA, IVK – Modified mineral mortar, group 3
were created according to EN 15804 and the building
3.8 Allocation context, respectively the product-specific
Mass allocation has been applied when primary data characteristics of performance, are taken into account.
have been used and implemented into the LCA model.
The GaBi 10 database SP40 (2020) was used.
3.9 Comparability
Basically, a comparison or an evaluation of EPD data
is only possible if all the data sets to be compared
4. LCA: Scenarios and additional technical information
Characteristic product properties
Information on biogenic carbon
The packaging material contains biogenic carbon
content which is presented below.
Information on describing the biogenic Carbon
Content at factury gate
Name Value Unit
Biogenic Carbon Content in product - kg C
Biogenic Carbon Content in
0.0194 kg C
accompanying packaging
For the preparation of building life cycle assessments,
it must be taken into account that in module A5
(installation in the building) the biogenic amount of CO
2
(0.0194 kg C *3.67 = 0.071 kg CO -eq.) of the
2
packaging bound in module A1-A3 is mathematically
booked out.
Transport to the building site (A4)
Name Value Unit
Transport distance 1000 km
Gross weight 34 - 40 t
Payload capacity 27 t
Installation into the building (A5)
Name Value Unit
Material loss 0.01 kg
Other resources for packaging material 0.055 kg
Water consumption 0.0003 m3
Material loss considers the amount of product not used
during the application phase into the building. This
amount is 1 % of the product, impacts related to the
production of this part are acounted to the A5 module.
This percentage is considered as waste to disposal
and impacts of its end of life have been considered into
the LCA model and declared in A5.
End of life (C1-C4)
Name Value Unit
Collected as mixed construction waste 1.128 kg
Landfilling 1.128 kg
The value above 1 kg is due to the use of water during
the installation phase where 50 % of water evaporate
while 50 % remain in the product.
7 Environmental Product Declaration DBC, EFCC, FEICA, IVK – Modified mineral mortar, group 3
5. LCA: Results
DESCRIPTION OF THE SYSTEM BOUNDARY (X = INCLUDED IN LCA; ND = MODULE OR INDICATOR NOT
DECLARED; MNR = MODULE NOT RELEVANT)
BENEFITS AND
CONSTRUCTI LOADS
PRODUCT STAGE ON PROCESS USE STAGE END OF LIFE STAGE BEYOND THE
STAGE SYSTEM
BOUNDARIES
8 Environmental Product Declaration DBC, EFCC, FEICA, IVK – Modified mineral mortar, group 3
lairetam
waR
ylppus tropsnarT
gnirutcafunaM
eht
morf
tropsnarT
etis
eht
ot
etag
ylbmessA esU
ecnanetniaM
riapeR
tnemecalpeR tnemhsibrufeR
ygrene
lanoitarepO esu
retaw
lanoitarepO esu
noitcurtsnoc-eD
noitilomed tropsnarT
gnissecorp
etsaW
lasopsiD -esueR -yrevoceR -gnilcyceR laitnetop
A1 A2 A3 A4 A5 B1 B2 B3 B4 B5 B6 B7 C1 C2 C3 C4 D
X X X X X ND ND MNR MNR MNR ND ND X X ND X X
RESULTS OF THE LCA - ENVIRONMENTAL IMPACT according to EN 15804+A2: 1 kg of modified mineral
mortar, group 3
Core Indicator Unit A1-A3 A4 A5 C1 C2 C4 D
GWP-total [kg CO2-Eq.] 1.62E+0 5.06E-2 1.16E-1 3.14E-4 1.40E-2 1.72E-2 -3.50E-2
GWP-fossil [kg CO2-Eq.] 1.68E+0 5.00E-2 2.48E-2 3.00E-4 1.33E-2 1.71E-2 -3.49E-2
GWP-biogenic [kg CO2-Eq.] -6.25E-2 1.46E-4 9.11E-2 1.39E-5 6.12E-4 5.41E-5 -8.21E-5
GWP-luluc [kg CO2-Eq.] 1.32E-3 4.05E-4 1.47E-5 7.21E-9 3.15E-7 4.92E-5 -2.45E-5
ODP [kg CFC11-Eq.] 1.31E-10 6.01E-18 1.31E-12 3.20E-20 1.40E-18 6.34E-17 -3.66E-16
AP [mol H+-Eq.] 4.83E-3 1.50E-4 6.53E-5 4.06E-6 4.21E-5 1.23E-4 -4.90E-5
EP-freshwater [kg P-Eq.] 2.48E-6 1.52E-7 3.05E-8 6.49E-11 2.83E-9 2.94E-8 -4.52E-8
EP-marine [kg N-Eq.] 9.91E-4 6.68E-5 1.54E-5 1.84E-6 1.93E-5 3.16E-5 -1.27E-5
EP-terrestrial [mol N-Eq.] 1.08E-2 7.48E-4 1.85E-4 2.02E-5 2.13E-4 3.47E-4 -1.36E-4
POCP [kg NMVOC-Eq.] 4.60E-3 1.32E-4 6.09E-5 5.54E-6 3.82E-5 9.56E-5 -3.64E-5
ADPE [kg Sb-Eq.] 1.78E-7 3.59E-9 2.00E-9 9.09E-12 3.97E-10 1.54E-9 -5.74E-9
ADPF [MJ] 3.57E+1 6.66E-1 3.82E-1 4.30E-3 1.88E-1 2.24E-1 -5.92E-1
[m³ world-Eq
WDP 1.54E-1 4.47E-4 2.49E-2 5.94E-7 2.59E-5 1.79E-3 -3.63E-3
deprived]
GWP = Global warming potential; ODP = Depletion potential of the stratospheric ozone layer; AP = Acidification potential of land and water; EP =
Caption Eutrophication potential; POCP = Formation potential of tropospheric ozone photochemical oxidants; ADPE = Abiotic depletion potential for non-
fossil resources; ADPF = Abiotic depletion potential for fossil resources; WDP = Water (user) deprivation potential
RESULTS OF THE LCA - INDICATORS TO DESCRIBE RESOURCE USE according to EN 15804+A2: 1 kg of
modified mineral mortar, group 3
Indicator Unit A1-A3 A4 A5 C1 C2 C4 D
PERE [MJ] 2.26E+0 3.74E-2 7.55E-1 1.35E-5 5.92E-4 2.94E-2 -1.30E-1
PERM [MJ] 7.21E-1 0.00E+0 -7.21E-1 0.00E+0 0.00E+0 0.00E+0 0.00E+0
PERT [MJ] 2.98E+0 3.74E-2 3.42E-2 1.35E-5 5.92E-4 2.94E-2 -1.30E-1
PENRE [MJ] 3.14E+1 6.67E-1 4.27E-1 4.30E-3 1.88E-1 2.25E-1 -5.92E-1
PENRM [MJ] 4.29E+0 0.00E+0 -8.66E-2 0.00E+0 0.00E+0 0.00E+0 0.00E+0
PENRT [MJ] 3.57E+1 6.67E-1 3.40E-1 4.30E-3 1.88E-1 2.25E-1 -5.92E-1
SM [kg] 0.00E+0 0.00E+0 0.00E+0 0.00E+0 0.00E+0 0.00E+0 0.00E+0
RSF [MJ] 0.00E+0 0.00E+0 0.00E+0 0.00E+0 0.00E+0 0.00E+0 0.00E+0
NRSF [MJ] 0.00E+0 0.00E+0 0.00E+0 0.00E+0 0.00E+0 0.00E+0 0.00E+0
FW [m³] 8.75E-3 4.33E-5 6.34E-4 2.43E-8 1.06E-6 5.66E-5 -1.50E-4
PERE = Use of renewable primary energy excluding renewable primary energy resources used as raw materials; PERM = Use of
renewable primary energy resources used as raw materials; PERT = Total use of renewable primary energy resources; PENRE = Use of
non-renewable primary energy excluding non-renewable primary energy resources used as raw materials; PENRM = Use of non-
Caption
renewable primary energy resources used as raw materials; PENRT = Total use of non-renewable primary energy resources; SM = Use
of secondary material; RSF = Use of renewable secondary fuels; NRSF = Use of non-renewable secondary fuels; FW = Use of net fresh
water
RESULTS OF THE LCA – WASTE CATEGORIES AND OUTPUT FLOWS according to EN 15804+A2:
1 kg of modified mineral mortar, group 3
Indicator Unit A1-A3 A4 A5 C1 C2 C4 D
HWD [kg] 1.42E-5 3.10E-8 1.43E-7 4.17E-13 1.82E-11 3.42E-9 -2.36E-10
NHWD [kg] 1.22E-1 1.02E-4 1.53E-2 4.40E-7 1.92E-5 1.13E+0 -2.74E-4
RWD [kg] 6.36E-4 8.25E-7 7.64E-6 4.62E-9 2.02E-7 2.56E-6 -4.43E-5
CRU [kg] 0.00E+0 0.00E+0 0.00E+0 0.00E+0 0.00E+0 0.00E+0 0.00E+0
MFR [kg] 0.00E+0 0.00E+0 0.00E+0 0.00E+0 0.00E+0 0.00E+0 0.00E+0
MER [kg] 0.00E+0 0.00E+0 0.00E+0 0.00E+0 0.00E+0 0.00E+0 0.00E+0
EEE [MJ] 0.00E+0 0.00E+0 1.48E-1 0.00E+0 0.00E+0 0.00E+0 0.00E+0
EET [MJ] 0.00E+0 0.00E+0 2.66E-1 0.00E+0 0.00E+0 0.00E+0 0.00E+0
HWD = Hazardous waste disposed; NHWD = Non-hazardous waste disposed; RWD = Radioactive waste disposed; CRU = Components
Caption for re-use; MFR = Materials for recycling; MER = Materials for energy recovery; EEE = Exported electrical energy; EET = Exported
thermal energy
RESULTS OF THE LCA – additional impact categories according to EN 15804+A2-optional:
1 kg of modified mineral mortar, group 3
Indicator Unit A1-A3 A4 A5 C1 C2 C4 D
[Disease
PM ND ND ND ND ND ND ND
Incidence]
[kBq U235-
IRP ND ND ND ND ND ND ND
Eq.]
ETP-fw [CTUe] ND ND ND ND ND ND ND
HTP-c [CTUh] ND ND ND ND ND ND ND
HTP-nc [CTUh] ND ND ND ND ND ND ND
SQP [-] ND ND ND ND ND ND ND
PM = Potential incidence of disease due to PM emissions; IR = Potential Human exposure efficiency relative to U235; ETP-fw = Potential
Caption comparative Toxic Unit for ecosystems; HTP-c = Potential comparative Toxic Unit for humans (cancerogenic); HTP-nc = Potential
comparative Toxic Unit for humans (not cancerogenic); SQP = Potential soil quality index
Potential Human exposure efficiency relative to U235, Disclaimer 1 – This impact category deals mainly with the
eventual impact of low dose ionizing radiation on human health of the nuclear fuel cycle. It does not consider
effects due to possible nuclear accidents, occupational exposure or radioactive waste disposal in underground
facilities. Potential ionizing radiation from the soil, radon and (from) some construction materials is also not
measured by this indicator.
ADP minerals & metals, ADP fossil, WDP, ETF-fw, HTP-c, HTP-nc, SQP, Disclaimer 2 – The results of this
environmental impact indicator shall be used with care as the uncertainties on these results are high or as there is
limited experience with the indicator.
Additional environmental impact indicators (suggested by EN15804, table 4) are not declared in the EPD. The
results of this environmental impact indicator shall be used with care as the uncertainties on these results are high
and as there is limited experience with the indicator (see ILCD classification in EN 15804, table 5). For this
reason, results based on these indicators are not considered suitable for a decision-making process and are thus
not declared in the EPD.
6. LCA: Interpretation
The majority of impacts are associated with the In all EPDs, CO is the most important contributor to
2
production phase (A1-A3). The most significant Global Warming Potential (GWP). For the Acidification
contribution to the production phase impacts is the Potential (AP), NOx and SO contribute the largest
2
upstream production of raw materials as the main share.
driver. Besides the cement also the dispersion powder Transportation to the construction site (A4) and the
influences the results significantly, although this is only installation process (A5) make a minor contribution to
used for up to 35 % of the total composition. Significant almost all impacts. The only exception is a relevant
contributions to Primary Energy Demand – Non- influence of carbon dioxide emissions in module A5 to
renewable (PENRT) derive from the energy resources Global Warming Potential (GWP) due to the
used in the production of raw materials. The largest incineration of the packaging materials plastic, paper
contributor to Primary Energy Demand – Renewable and pallets.
(PERT) is the consumption of renewable energy In module A4, transport to construction site, values for
resources required for the generation and supply of Eutrophication (freshwater, marine and terrestrial)
electricity. During manufacturing (A1-A3) some have an impact due principally to the emission of
influence also arises due to the wooden pallets and phosphate. Furthermore, climate change from land use
paper used as packaging that need solar energy for change is influenced by transport processes, due to
photosynthesis. It should be noted that Primary Energy the diesel production used as fuel, because part of this
Demand – Renewable (PERT) generally represents a diesel has been produced from bio-based raw
small percentage of the production phase primary materials.
energy demand with the bulk of the demand coming The end-of-life phases have a negligible influence on
from non-renewable energy resources. all impacts.
7. Requisite evidence
Leaching If of relevance for the application (usually if the
Special tests and evidence have not been carried out products are used outside of buildings) the leaching
or provided within the framework of drawing up this behaviour has to be measured e.g. according to DIN
Model EPD. Some member states require special EN 12457/1­­4 or DIN EN 14405 combined with the
documentation on leaching for specific areas of Council decision 2003/33/EC.
application. This documentation has to be provided
separately and is specific to the product in question.
8. References
EN 998-1 EN 998-1:2016, Specification for mortar for masonry –
Part 1: Rendering and plastering mortar
9 Environmental Product Declaration DBC, EFCC, FEICA, IVK – Modified mineral mortar, group 3
EN 13279
EN 1015-17 EN 13279-1:2008, Gypsum binders and gypsum
EN 1015-17:2005-01, Methods of test for mortar for plasters – Part 1: Definitions and requirements
masonry – Part 17: Determination of water-soluble
chloride content of fresh mortars EN 13501-1
EN 13501-1:2018, Fire classification of construction
EN 1504-3 products and building products – Part 1: Classification
EN 1504-3:2005-12, Products and systems for the using data from reaction to fire tests
protection and repair of concrete structures –
Definitions, requirements, quality control and EN 13813
evaluation of conformity – Part 3: Structural and non- EN 13813:2002-10, Screed material and floor screeds
structural repair – Screed materials – Properties and requirements
EN 1504-7 EN 13888
EN 1504-7:2006-08, Products and systems for the EN 13888:2009, Grout for tiles – Requirements,
protection and repair of concrete structures – evaluation of conformity, classification and designation
Definitions, requirements, quality control and
evaluation of conformity – Part 7: Reinforcement EN 13892-8
corrosion protection EN 13892-8:2003-02, Methods of test for screed
materials – Part 8: Determination of bond strength
EN 1542
EN 1542:1999-07, Products and systems for the ISO 14025
protection and repair of concrete structures – Test DIN EN ISO 14025:2011-10, Environmental labels and
methods – Measurement of bond strength by pull-off declarations — Type III environmental declarations —
Principles and procedures
EN 12004
EN 12004:2012, Adhesives for tiles – Requirements, DIN EN 14405
evaluation of conformity, classification and designation DIN EN 14405:2017-05, Characterization of waste -
Leaching behaviour test - Up-flow percolation test
EN 12004-2 (under specified conditions)
EN 12004-2:2017, Adhesives for ceramic tiles - Part 2:
Test methods EN 14891
EN 14891:2012-04, Liquid-applied water impermeable
EN 12190 products for use beneath ceramic tiling bonded with
EN 12190:1998-12, Products and systems for the adhesives – Requirements, test methods, evaluation of
protection and repair of concrete structures – Test conformity, classification and designation
methods – Determination of compressive strength of
repair mortar EN 15183
EN 15183:2006-11, Products and systems for the
DIN EN 12457-1 protection and repair of concrete structures – Test
DIN EN 12457-1:2003-01, Characterization of waste - methods – Corrosion protection test
Leaching; Compliance test for leaching of granular and
sludges - Part 1: One stage batch test at a liquid to EN 15804
solid ration of 2 l/kg with particle size below 4 mm EN 15804+A2+AC:2021, Sustainability of construction
(without or with size reduction) works — Environmental Product Declarations — Core
rules for the product category of construction products
DIN EN 12457-2
DIN EN 12457-2:2003-01, Characterization of waste - EAD 030295-00-0605
Leaching; Compliance test for leaching of granular and EAD 030295-00-0605, Flexible polymer modified
sludges - Part 2: One stage batch test at a liquid to mineral thick coating
solid ratio of 10 l/kg with particle size below 4 mm
(without or with size reduction) EAD 030352-00-0503
EAD 030352-00-0503:2019:01, Liquid applied
watertight covering kits for wet room floors and/or walls
DIN EN 12457-3
DIN EN 12457-3:2021-03, Characterization of waste - EAD 040083-00-0404
Leaching - Compliance test for leaching of granular EAD 040083-00-0404:2013, External Thermal
waste materials and sludges - Part 3: Two stage batch Insulation Composite Systems with Rendering
test at a liquid to solid ratio of 2 l/kg and 8 l/kg for
materials with high solid content with particle size 96/603/EC
below 4 mm (without or with size reduction) Commission decision of 4 October 1996 for specifying
a directory of products to be classified as category A
"No contribution to fire" in accordance with decision
DIN EN 12457-4 94/611/EC on construction products for implementing
DIN EN 12457-4:2003-01, Characterization of waste - Article 20 of Directive 89/106/EEC
Leaching; Compliance test for leaching of granular
waste materials and sludges - Part 4: One stage batch 2000/532/EC
test at a liquid to solid ratio of 10 l/kg for materials with Commission decision dated 3 May 2000 replacing
particle size below 10 mm (without or with limited size decision 94/3/EC on a waste directory in accordance
reduction) with Article 1 a) of Council Directive 75/442/EEC on
waste and Council decision 94/904/EC on a directory
10 Environmental Product Declaration DBC, EFCC, FEICA, IVK – Modified mineral mortar, group 3
of hazardous waste in terms of Article 1, paragraph 4 GaBi 10 documentation
of Directive 91/689/EEC on hazardous waste Gabi 10: documentation of GaBi 10 data sets from the
data base for Life Cycle Engineering LBP, University of
2003/33/EC: Stuttgart and Sphera, http://documentation.gabi-
Council Decision of 19 December 2002 establishing software.com/, 2020
criteria and procedures for the acceptance of waste at
landfills pursuant to Article 16 of and Annex II to IBU 2021
Directive 1999/31/EC Institut Bauen und Umwelt e.V.: General Instructions
for the EPD programme of Institut Bauen und Umwelt
Candidate list e.V. EPD programme. Version 2.0. Berlin: Institut
Candidate List of substances of very high concern for Bauen und Umwelt e.V., 2021
Authorisation, published in accordance with Article www.ibu-epd.com
59(10) of the REACH Regulation, ECHA,
www.echa.europa.eu/candidate-list-table MVV TB
Ü-mark in accordance with ‘Model Administrative
CPR Order laying down Technical Building Regulations’
CPR Regulation (EU) No 305/2011 of the European (MVV TB) no. C 2.1.4.5
Parliament and of the Council of 9 March 2011 laying
down harmonised conditions for the marketing of PCR Part A
construction products and repealing Council Directive Product Category Rules for Building-Related Products
89/106/EEC and Services, Part A: Calculation Rules for the Life
Cycle Assessment and Requirements on the Project
DAfStb Guideline report, Version 1.1, Institut Bauen und Umwelt e.V.,
DAfStb Guideline on ‘Production and use of cement- 2021-01
bound flow concrete and grouting mortar’ (VeBMR),
2019-07 PCR Part B
Product Category Rules for Construction Products,
Decopaint Directive Part B: Mineral Factory-Made Mortars, 2017-11
Directive 2004/42/CE of the European Parliament and
the council of 21 April 2004 on the limitation of PG AIV
emissions of volatile organic compounds due to the Testing principles regarding the issuing of general
use of organic solvents in certain paints and varnishes building authority test certificates for waterproofing with
and vehicle refinishing products and amending waterproofing in conjunction with ceramic tiles (PG-
Directive 1999/13/EC AIV:2018-03)
EWC 101314 PG MDS/FPD
2000/532/EC European Waste Catalogue / Ordinance Testing principles regarding the issuing of general
on European List of Wastes: Waste concrete and building authority test certificates for waterproofing with
concrete sludge mineral waterproofing slurries and flexible polymer
thick coatings (PG-MDS/FPD:2016-11)
EWC 170101
2000/532/EC European Waste Catalogue / Ordinance REACH
on European List of Wastes: Concrete Directive (EG) No. 1907/2006 of the European
Parliament and of the Council dated 18 December
EWC 170107 2006 on the registration, evaluation, approval and
2000/532/EC European Waste Catalogue / Ordinance restriction of chemical substances (REACH), for
on European List of Wastes: Mixtures of concrete, establishing a European Agency for chemical
bricks, tiles and ceramics substances, for amending Directive 1999/45/EC and
for annulment of Directive (EEC) No. 793/93 of the
EWC 170802 Council, Directive (EC) No. 1488/94 of the
2000/532/EC European Waste Catalogue / Ordinance Commission, Guideline 76/769/EEC of the Council and
on European List of Wastes: Gypsum based Guidelines 91/155/EEC, 93/67/EEC, 93/105/EC and
construction metals e.g. for plasterboard 2000/21/EC of the Commission.
GaBi 10
GaBi 10: Software and database for comprehensive
analysis. LBP, University of Stuttgart and Sphera, 2020
11 Environmental Product Declaration DBC, EFCC, FEICA, IVK – Modified mineral mortar, group 3
Publisher
Institut Bauen und Umwelt e.V. Tel +49 (0)30 3087748- 0
Hegelplatz 1 Fax +49 (0)30 3087748- 29
10117 Berlin Mail info@ibu-epd.com
Germany Web www.ibu-epd.com
Programme holder
Institut Bauen und Umwelt e.V. Tel +49 (0)30 - 3087748- 0
Hegelplatz 1 Fax +49 (0)30 – 3087748 - 29
10117 Berlin Mail info@ibu-epd.com
Germany Web www.ibu-epd.com
Author of the Life Cycle
Assessment Tel +49 711 341817-0
Sphera Solutions GmbH Fax +49 711 341817-25
Hauptstraße 111- 113 Mail info@sphera.com
70771 Leinfelden-Echterdingen Web www.sphera.com
Germany
Owner of the Declaration
FEICA - Association of the Tel +32 (0)267 673 20
European Adhesive and Sealant Fax +32 (0)267 673 99
Industry Mail info@feica.eu
Rue Belliard 40 box 10 Web www.feica.eu
1040 Brussels
Belgium
Tel +49 (0)211 67931-10
Fax +49 (0)211 67931-33
Industrieverband Klebstoffe e.V Mail info@klebstoffe.com
Völklinger Straße 4 Web www.klebstoffe.com
40219 Düsseldorf
Germany
Tel +32289720-39
Fax +32289720-37
EFCC - European Federation for Mail info@efcc.be
Construction Chemicals Web www.efcc.eu
Boulevard du Triomphe 172
1160 Brussels
Belgium
Tel +49 (0)69 2556-1318
Fax +49 (0)69 2556-1319
Mail info@deutsche-bauchemie.de
Deutsche Bauchemie e.V. Web www.deutsche-bauchemie.de
Mainzer Landstr. 55
60329 Frankfurt
Germany
