ENVIRONMENTAL PRODUCT DECLARATION
as per ISO 14025 and EN 15804+A2
Owner of the Declaration dormakaba International Holding GmbH
Publisher Institut Bauen und Umwelt e.V. (IBU)
Programme holder Institut Bauen und Umwelt e.V. (IBU)
Declaration number EPD-DOR-20210320-CBA1-EN
Issue date 04.05.2022
Valid to 03.05.2027
BEST T Deadbolt Series
dormakaba
www.ibu-epd.com | https://epd-online.com
General Information
dormakaba BEST T Deadbolt Series
Programme holder Owner of the declaration
IBU – Institut Bauen und Umwelt e.V. dormakaba International Holding GmbH
Hegelplatz 1 DORMA Platz 1
10117 Berlin 58256 Ennepetal
Germany Germany
Declaration number Declared product / declared unit
EPD-DOR-20210320-CBA1-EN 1 lock (1 piece) of the BEST T Deadbolt Series.
This declaration is based on the product category rules: Scope:
Building Hardware products, 01.08.2021 This Environmental Product Declaration refers to a specific lock
(PCR checked and approved by the SVR) manufactured by dormakaba. The production site is located in Indianapolis
(USA).
Issue date The data represents the year 2020.
The owner of the declaration shall be liable for the underlying information
04.05.2022
and evidence; the IBU shall not be liable with respect to manufacturer
information, life cycle assessment data and evidences.
Valid to
The EPD was created according to the specifications of EN 15804+A2. In
03.05.2027 the following, the standard will be simplified as EN 15804.
Verification
The standard EN 15804 serves as the core PCR
Independent verification of the declaration and data according to ISO
14025:2011
internally X externally
Dipl.-Ing. Hans Peters
(Chairman of Institut Bauen und Umwelt e.V.)
Florian Pronold Dr.-Ing. Wolfram Trinius,
(Managing Director Institut Bauen und Umwelt e.V.) (Independent verifier)
1 Environmental Product Declaration - dormakaba - BEST T Deadbolt Series
Product
Performance data of the product with respect to its
Product description/Product definition characteristics in accordance with the relevant technical
Built with identical tubular assemblies, the 8T both fit standard provision which can be applied are mentioned above.
door preps. The 8T is often paired with a cylindrical lock in
commercial office spaces, residential applications and other Base materials/Ancillary materials
spaces where there is a greater need for security and, more The major material composition including the packaging of the
specifically, a deadbolt that is more resistant to brute force product are listed below.
attack. The 8T is also available with lead line options, making it Name Value Unit
a good solution for radioactive doors (MRI, x-ray, etc.) in
Brass 77 %
healthcare facilities. For the use and application of the product
Paper 9 %
the respective national provisions at the place of use apply. The
HD8000 is a Underwriters Laboratories (UL) listed product. Stainless steel 7 %
The standards which can be applied are the following: Steel 7 %
• ANSI/BHMA A156.36 Plastics <1 %
• UL/ULC listed
The product/s include/s partial articles which contain
• ANSI/ICC A117.1
substances listed in the Candidate List of REACH Regulation
1907/2006/EC (date: 17.01.2022) exceeding 0.1 percentage by
Application
mass: no
The BEST T Deadbolt Series can be used in following building
types: Reference service life
• Healtcare The reference service life of the T Deadbolt Series lock
• Retail and commercial depends on the traffic pattern and degree of usage of the door.
These locks are rated to ANSI Grade 1, meaning they are
Technical Data designed to withstand a minimum of 1,000,000 cycles.
The lock has following technical properties:
LCA: Calculation rules
Construction stage - Modules A4-A5
Declared Unit The construction process stage includes:
The declared unit is 1 piece of the product: BEST T Deadbolt — A4, transport to the building site;
Series. — A5, installation into the building;
Declared unit including provision of all materials, products and energy, as well
as waste processing up to the end-of waste state or disposal of
Name Value Unit
final residues during the construction process stage.
Declared unit 1 piece/product
Mass of declared Product 1.26 kg End-of-life stage– Modules C1-C4 and D
The end-of-life stage includes:
System boundary — C1, de-construction, demolition:
The type of EPD is: cradle to gate with options, modules C1– — C2, transport to waste processing;
C4, and module D (A1–A3 + C + D and additional modules: A4 — C3, waste processing for reuse, recovery and/or recycling;
+ A5) — C4, disposal;
including provision and all transport, provision of all materials,
Production - Module A1-A3 products and related energy and water use.
The product stage includes:
— A1, raw material extraction, processing and mechanical Module D (Benefits and loads beyond the system boundary)
treatments, processing of secondary material input (e.g. includes:
recycling processes), — A2, transport to the manufacturer, — D, recycling potentials, expressed as net impacts and
— A3, manufacturing and assembly including provision of all benefits.
materials, products and energy, as well as waste processing up
to the end-of waste state.
2 Environmental Product Declaration - dormakaba - BEST T Deadbolt Series
Geographic Representativeness Comparability
Land or region, in which the declared product system is Basically, a comparison or an evaluation of EPD data is only
manufactured, used or handled at the end of the product´s possible if all the data sets to be compared were created
lifespan: North America according to EN 15804 and the building context, respectively
the product-specific characteristics of performance, are taken
into account.
LCA: Scenarios and additional technical information
Installation into the building (A5)
Characteristic product properties of biogenic carbon
Name ValueUnit
Information on describing the biogenic Carbon Content at
Output substances following waste treatment on
factory gate 0.107 kg
site (packaging)
Name Value Unit
Biogenic carbon content in product - kg C End of life (C1-C4)
C1: The product dismantling from the building is done manually
Note: 1 kg of biogenic carbon is equivalent to 44/12 kg of CO .
2 without environmental burden.
C2: Transport to waste treatment at end of life is 50km.
Additional technical information for the declared modules. Name Value Unit
Collected separately waste type 1.14 kg
Transport to the building site (A4)
Recycling 1.14 kg
Name Value Unit
Energy recovery 0.0068 kg
Litres of fuel per 1 kg (truck) 0.00276l/100km
Final deposition 0,002 kg
Transport distance (truck) 1500 km
Capacity utilisation (including empty runs) Reuse, recovery and/or recycling potentials (D), relevant
55 %
average scenario information
Transport distance (ship) 10000 km Name Value Unit
Collection rate is 100%.
3 Environmental Product Declaration - dormakaba - BEST T Deadbolt Series
LCA: Results
Disclaimer:
EP-freshwater: This indicator has been calculated as 'kg P eq' as required in the characterization model (EUTREND model, Struijs et
al., 2009b, as implemented in ReCiPe; http://eplca.jrc.ec.europa.eu/LCDN/developerEF.xhtml)
DESCRIPTION OF THE SYSTEM BOUNDARY (X = INCLUDED IN LCA; MND = MODULE OR INDICATOR NOT DECLARED; MNR
= MODULE NOT RELEVANT)
Benefits and
Construction loads beyond
Product stage Use stage End of life stage
process stage the system
boundaries
la ire ta m w a Ry lp p u s tro p s n a rT g n iru tc a fu n a M e h t m o rf tro p s n a rTe tis e h t o t e ta g y lb m e s s A e s U e c n a n e tn ia M ria p e R tn e m e c a lp e R tn e m h s ib ru fe R y g re n e la n o ita re p Oe s u re ta w la n o ita re p Oe s u n o itc u rts n o c -e Dn o itilo m e d tro p s n a rT g n is s e c o rp e ts a W la s o p s iD -e s u e R-y re v o c e R-g n ilc y c e Rla itn e to p
A1 A2 A3 A4 A5 B1 B2 B3 B4 B5 B6 B7 C1 C2 C3 C4 D
X X X X X MND MND MNR MNR MNR X MND X X X X X
RESULTS OF THE LCA - ENVIRONMENTAL IMPACT according to EN 15804+A2: 1 lock
Parameter Unit A1-A3 A4 A5 B6 C1 C2 C3 C4 D
GWP-total kg CO 2 eq 2.49E+00 2.05E-01 2.74E-01 0 0 5E-03 1.7E-02 3.05E-06 -5.5E-01
GWP-fossil kg CO 2 eq 2.47E+00 1.98E-01 2.74E-01 0 0 5E-03 1.7E-02 3.03E-06 -5.51E-01
GWP-biogenic kg CO 2 eq 1.2E-02 7E-03 6.38E-06 0 0 2.22E-04 4.03E-07 1.04E-08 1E-03
GWP-luluc kg CO 2 eq 3.34E-03 4.57E-06 1.55E-05 0 0 1.14E-07 9.77E-07 8.73E-09 -7.12E-04
ODP kg CFC11 eq 2.15E-14 2.04E-17 1.38E-16 0 0 5.06E-19 8.72E-18 1.13E-20 -1.5E-15
AP mol H+ eq 1.59E-02 2E-03 4.88E-05 0 0 4.8E-06 3.08E-06 2.18E-08 -7.12E-04
EP-freshwater kg P eq 3.76E-06 4.28E-08 2.2E-08 0 0 1.03E-09 1.39E-09 5.21E-12 -2.84E-07
EP-marine kg N eq 1.21E-03 4.47E-04 1.1E-05 0 0 1.53E-06 6.94E-07 5.6E-09 -2.78E-04
EP-terrestrial mol N eq 1.71E-02 5E-03 2.22E-04 0 0 1.7E-05 1.4E-05 6.16E-08 -3E-03
kg NMVOC
POCP 4.62E-03 1E-03 3.04E-05 0 0 4.32E-06 1.92E-06 1.7E-08 -8.32E-04
eq
ADPE kg Sb eq 4.82E-04 5.75E-09 1.89E-09 0 0 1.44E-10 1.2E-10 2.73E-13 1.31E-04
ADPF MJ 3.82E+01 2.72E+00 1.27E-01 0 0 6.8E-02 8E-03 3.98E-05 -6.96E+00
m3 world eq
WDP 6.87E-01 3.81E-04 2.8E-02 0 0 9.4E-06 2E-03 3.18E-07 -1.36E-01
deprived
GWP = Global warming potential; ODP = Depletion potential of the stratospheric ozone layer; AP = Acidification potential of land and water; EP =
Eutrophication potential; POCP = Formation potential of tropospheric ozone photochemical oxidants; ADPE = Abiotic depletion potential for non-fossil
resources; ADPF = Abiotic depletion potential for fossil resources; WDP = Water (user) deprivation potential)
RESULTS OF THE LCA - INDICATORS TO DESCRIBE RESOURCE USE according to EN 15804+A2: 1 lock
Parameter Unit A1-A3 A4 A5 B6 C1 C2 C3 C4 D
PERE MJ 7.81E+00 9E-03 3.3E-02 0 0 2.15E-04 4E-03 5.21E-06 -1.07E+00
PERM MJ 2E-03 0 0 0 0 0 -2E-03 0 0
PERT MJ 7.81E+00 9E-03 3.3E-02 0 0 2.15E-04 2E-03 5.21E-06 -1.07E+00
PENRE MJ 3.34E+01 2.72E+00 4.76E+00 0 0 6.8E-02 1.97E-01 3.98E-05 -6.96E+00
PENRM MJ 4.82E+00 0 -4.63E+00 0 0 0 -1.89E-01 0 0
PENRT MJ 3.82E+01 2.72E+00 1.27E-01 0 0 6.8E-02 8E-03 3.98E-05 -6.96E+00
SM kg 1.07E+00 0 0 0 0 0 0 0 0
RSF MJ 0 0 0 0 0 0 0 0 0
NRSF MJ 0 0 0 0 0 0 0 0 0
FW m3 2.1E-02 1.55E-05 6.7E-04 0 0 3.85E-07 4.23E-05 1E-08 -7E-03
PERE = Use of renewable primary energy excluding renewable primary energy resources used as raw materials; PERM = Use of renewable primary
energy resources used as raw materials; PERT = Total use of renewable primary energy resources; PENRE = Use of non-renewable primary energy
excluding non-renewable primary energy resources used as raw materials; PENRM = Use of non-renewable primary energy resources used as raw
materials; PENRT = Total use of non-renewable primary energy resources; SM = Use of secondary material; RSF = Use of renewable secondary fuels;
NRSF = Use of non-renewable secondary fuels; FW = Use of net fresh water
RESULTS OF THE LCA – WASTE CATEGORIES AND OUTPUT FLOWS according to EN 15804+A2:
1 lock
Parameter Unit A1-A3 A4 A5 B6 C1 C2 C3 C4 D
HWD kg 8.98E-08 2.65E-10 4.84E-10 0 0 6.6E-12 3.05E-11 6.07E-13 -1.25E-07
NHWD kg 3.42E-01 2.78E-04 2.8E-02 0 0 6.96E-06 2E-03 2E-04 -2.2E-02
RWD kg 1.5E-03 2.94E-06 4.71E-06 0 0 7.31E-08 2.97E-07 4.53E-10 -1.3E-04
CRU kg 0 0 0 0 0 0 0 0 0
MFR kg 0 0 0 0 0 0 1.14E+00 0 0
MER kg 0 0 0 0 0 0 0 0 0
4 Environmental Product Declaration - dormakaba - BEST T Deadbolt Series
EEE MJ 1.7E-02 0 5.07E-01 0 0 0 0 0 0
EET MJ 3.1E-02 0 1.16E+00 0 0 0 0 0 0
HWD = Hazardous waste disposed; NHWD = Non-hazardous waste disposed; RWD = Radioactive waste disposed; CRU = Components for re-use;
MFR = Materials for recycling; MER = Materials for energy recovery; EEE = Exported electrical energy; EET = Exported thermal energy
RESULTS OF THE LCA – additional impact categories according to EN 15804+A2-optional:
1 lock
Parameter Unit A1-A3 A4 A5 B6 C1 C2 C3 C4 D
Disease
PM 1.52E-07 2.65E-08 6.22E-10 0 0 2.52E-11 3.93E-11 2.69E-13 -2.93E-08
incidence
IR kBq U235 eq 2.57E-01 4.21E-04 4.24E-04 0 0 1.04E-05 2.68E-05 4.66E-08 -2.7E-02
ETP-fw CTUe 2.26E+01 1.93E+00 4.8E-02 0 0 4.8E-02 3E-03 2.27E-05 -1.49E+00
HTP-c CTUh 1.26E-07 3.62E-11 4.12E-12 0 0 9.07E-13 2.6E-13 3.37E-15 -6.7E-10
HTP-nc CTUh 6.43E-08 1.58E-09 4.18E-10 0 0 3.88E-11 2.64E-11 3.71E-13 1.15E-08
SQP SQP 1E+01 7E-03 3.8E-02 0 0 1.75E-04 2E-03 8.3E-06 -1.26E-01
PM = Potential incidence of disease due to PM emissions; IR = Potential Human exposure efficiency relative to U235; ETP-fw = Potential comparative
Toxic Unit for ecosystems; HTP-c = Potential comparative Toxic Unit for humans (cancerogenic); HTP-nc = Potential comparative Toxic Unit for humans
(not cancerogenic); SQP = Potential soil quality index
Disclaimer 1 – for the indicator “Potential Human exposure efficiency relative to U235”. This impact category deals mainly with the
eventual impact of low-dose ionizing radiation on human health of the nuclear fuel cycle. It does not consider effects due to possible
nuclear accidents, occupational exposure or radioactive waste disposal in underground facilities. Potential ionizing radiation from the
soil, radon and from some construction materials is also not measured by this indicator.
Disclaimer 2 – for the indicators “abiotic depletion potential for non-fossil resources”, “abiotic depletion potential for fossil resources”,
“water (user) deprivation potential, deprivation-weighted water consumption”, “potential comparative toxic unit for ecosystems”,
“potential comparative toxic unit for humans – cancerogenic”, “Potential comparative toxic unit for humans - not cancerogenic”,
“potential soil quality index”. The results of this environmental impact indicator shall be used with care as the uncertainties on these
results are high as there is limited experience with the indicator.
References
ANSI/ICC A117.1 for Life Cycle Engineering 1992-2020 Version 10.0.0.71
ANSI/ICC A117.1 - 2017, Accessible and usable buildings and University of Stuttgart Leinfelden-Echterdingen.
facilities.
GaBi ts documentation
ANSI/BHMA A156.36 GaBi life cycle inventory data documentation (https://www.gabi-
ANSI/BHMA A156.4 - 2016, Auxiliary Locks. software.com/support/gabi/gabidatabase- 2020-lci-
documentation/).
ECHA
European Chemicals Agency: https://echa.europa.eu/de/home. LCA-tool dormakaba
LCA-tool, IBU-DOR-202104-LT1-EN.
REACH Developed by Sphera Solutions GmbH.
Registration, Evaluation, Authorisation and Restriction of
Chemicals (REACH), Regulation (EC) No 1907/2006. PCR Part A
PCR – Part A: Calculation Rules for the Life Cycle Assessment
EN 15804:2019+A2 and Requirements on the Project Report according to EN
EN 15804:2019+A2 (in press), Sustainability of construction 15804+A2:2019, Version 1.0, 2020, Institut Bauen und Umwelt
works — Environmental Product Declarations — Core rules for e.V., www.ibu-epd.com.
the product category of construction products.
PCR Part B
Further References PCR – Part B: Requirements on the EPD for Building
Hardware product, version 1.2, Institut Bauen und
IBU Umwelt e.V., www.ibu-epd.com, 2017.
Institut Bauen und Umwelt e.V.: General Instructions for the
EPDs programme of Institut Bauen und Umwelt e.V. Version UL
2.0., Berlin: Institut Bauen und Umwelt e.V., 2021. www.ibu- Underwriters Laboratories,
epd.com. https://www.ul.com/.
GaBi ULC
Sphera Solutions GmbH Gabi Software System and Database Underwriters Laboratories of Canada,https://canada.ul.com/.
5 Environmental Product Declaration - dormakaba - BEST T Deadbolt Series
Publisher
Institut Bauen und Umwelt e.V. +49 (0)30 3087748- 0
Hegelplatz 1 info@ibu-epd.com
10117 Berlin www.ibu-epd.com
Germany
Programme holder
Institut Bauen und Umwelt e.V. +49 (0)30 3087748- 0
Hegelplatz 1 info@ibu-epd.com
10117 Berlin www.ibu-epd.com
Germany
Author of the Life Cycle Assessment
Sphera Solutions GmbH +49 711 341817-0
Hauptstraße 111- 113 info@sphera.com
70771 Leinfelden-Echterdingen www.sphera.com
Germany
Owner of the Declaration
dormakaba International Holding GmbH +49 2333 793-0
DORMA Platz 1 info.de@dormakaba.com
58256 Ennepetal www.dormakaba.com
Germany
6 Environmental Product Declaration - dormakaba - BEST T Deadbolt Series
