ENVIRONMENTAL PRODUCT DECLARATION
as per ISO 14025 and EN 15804+A2
Owner of the Declaration VELUX Group
Publisher Institut Bauen und Umwelt e.V. (IBU)
Programme holder Institut Bauen und Umwelt e.V. (IBU)
Declaration number EPD-VEL-20220141-IBJ3-EN
Issue date 25.07.2022
Valid to 24.07.2027
VELUX flat roof window CVU - solar-powered
VELUX A/S
www.ibu-epd.com | https://epd-online.com
1. General Information
VELUX A/S VELUX flat roof window CVU - solar-powered
Programme holder Owner of the declaration
IBU – Institut Bauen und Umwelt e.V. VELUX Group
Hegelplatz 1 Ådalsvej 99
10117 Berlin 2970 Hørsholm
Germany Denmark
Declaration number Declared product / declared unit
EPD-VEL-20220141-IBJ3-EN The declaration represents 1 piece of a solar-powered VELUX flat roof
window CVU of the size 1.20 m x 1.20 m = 1.44 m2
This declaration is based on the product category rules: Scope:
Windows and doors , 01.08.2021 The declaration covers 100% of solar-powered VELUX flat roof windows
(PCR checked and approved by the SVR) CVU by Østbirk Bygningsindustri, Denmark.
The owner of the declaration shall be liable for the underlying information
and evidence; the IBU shall not be liable with respect to manufacturer
Issue date information, life cycle assessment data and evidences.
25.07.2022
The EPD was created according to the specifications of EN 15804+A2. In
the following, the standard will be simplified as EN 15804.
Valid to
Verification
24.07.2027
The standard EN 15804 serves as the core PCR
Independent verification of the declaration and data according to ISO
14025:2011
internally X externally
Dipl.-Ing. Hans Peters
(Chairman of Institut Bauen und Umwelt e.V.)
Florian Pronold Dr. Eva Schmincke,
(Managing Director Institut Bauen und Umwelt e.V.) (Independent verifier)
1 Environmental Product Declaration - VELUX A/S - VELUX flat roof window CVU - solar-powered
2. Product
• EAD 220062-00-0401, June 2017, rooflight with bonded
2.1 Product description/Product definition
or mechanically fastened cover glass.
The solar-powered Velux flat roof windows CVU consists of a
motorised base unit made of a PUR/GRP curb with a wooden 2.4 Delivery status
core, with integrated glazing unit and hinges on one side to
The product is available in pre-defined sizes covering 0,6x0,6m
allow for venting and a single layer flat or curved glass top unit
to 1,5x1,5m.
on top. For the placing of the product on the market in the
European Union/European Free Trade Association /EU/EFTA) 2.5 Base materials/Ancillary materials
(with the exception of Switzerland) the Regulation (EU) No. Composition of the base unit CVU:
305/2011 (CPR) applies. The product needs a declaration of polyurethane 7 %
performance taking into consideration EAD 220062-00-0401, heat-treated wood 8 %
June 2017, rooflight with bonded or mechanically fastened galvanized steel 7 %
cover glass and the CE-marking. For the application and use PU with glass fibres 13 %
the respective national provisions apply. laminated glass 25 %
tempered glass 12 %
2.2 Application
heat strenghtened glass 15 %
Velux flat roof windows CVU are used in renovation and new
others
build.
Composition of the top unit (ISU 1093):
2.3 Technical Data
Curved glass 73 %
The Declaration of Performance including relevant technical
Aluminium 25 %
specifications and test methods/test standards can be
others
downloaded from the website www.velux.com/ce.
Composition of the motor (CVP solar):
The declared values in the table relate to the reference product
glavanized steel 15 %
incl. an average pane. For other covered product variants,
iron/cast iron 20 %
specific values can be selected at the bottom of the above-
steel 15 %
mentioned download page
PET/PC/PA 10 %
Constructional data for CVU 120120 20+ISU 1093 cables 10 %
For other variants, see velux.com/ce DC motor 8 %
Name Value Unit solar cell 5 %
battery 10 %
Resistance to fire EN
NPD - others
13501-2
External fire
1) 'This product/article/at least one partial article contains
performance EN NPD -
substances listed in the candidate list (date: 02.03.2022)
13501-5
exceeding 0.1 percentage by mass:
Water tightness EN
9A Class • no
1873
2) 'This product/article/at least one partial article contains other
Resistance to wind
C3 Class CMR substances in categories 1A or 1B which are not on the
load
candidate list, exceeding 0.1 percentage by mass:
5 mm toughened/ -- / 4 mm
Resistance to snow • not investigated with suppliers
toughened / 16 mm / 7.5 mm -
load 3) 'Biocide products were added to this construction product or
(33.4) laminated float
it has been treated with biocide products (this then concerns a
Impact resistance 3 Class
treated product as defined by the (EU) Regulation on Biocidal
Bonding of cover Products No. 528/2012):
Compliant (ΔX≥0.75) -
glass
• no
Airborne sound
insulation EN ISO 39 (-1;-5) dB Recycled content
410-3
Thermal
Urc,ref300: 0,65 W/(m2K)
transmittance EN -
Arc,ref300: 4,4 m2
1873
Total solar energy
0,52 -
transmittance
Light transmittance
0,69 - The values stated in the table relate to the recycled material
EN 410
streams in VELUX production.
Frame factor 0,1 -
Air permeability EN
4 Class
1026 2.6 Manufacture
Base unit:
Performance data of the product in accordance with the
declaration of performance with respect to its essential
The PU raw material, gaskets and other minor components are
characteristics according to
produced outside Velux.
2 Environmental Product Declaration - VELUX A/S - VELUX flat roof window CVU - solar-powered
Cutting and profiling of wood reinforcements are done at hazards to water, air and soil cannot arise when the products
production sites in Polen and Denmark. are used as intended.
The PUR/GRP curb with wooden core, the insulating glass unit, Health protection: According to current knowledge, no health
the motor and the wall switch are assembled at the production hazards or impairments are to be expected.
site in Denmark.
2.12 Reference service life
The production and final assembly of the base unit takes place It is not possible to calculate the reference service life
at the production site in Denmark. according to ISO 15686. The service life based on a
manufacturer's declaration is 30 years. The corresponding
The final production processes includes preparation of the utilization scenario is declared in 4.
PU/wood frame by cutting and profiling of wood, moulding,
2.13 Extraordinary effects
cutting, sandblasting and painting, assembly of the GRP sash
by pultrusion, profiling and drilling, cutting and mounting of Fire
gaskets and installation of the glazing unit and window opener
as well as packaging, stacking and wrapping of the product on Fire performance according to EN 13501:1
pallets.
Name Value
Building material class D
Top-unit:
Burning droplets s2
All raw materials and components are produced outside Velux. Smoke gas development d2
The glass top unit is assembled at the production site in
Water
Slovakia.
In the event of unforeseen exposure to water (flood), VELUX
flat roof windows must be replaced as electrical components;
The final production processes include assembly of product, as
no adverse effects on human health or the environment are to
well as packaging, stacking and wrapping of the product on
be expected.
pallets.
The factories are ISO 9001 certified.
Mechanical destruction
In the event of unforeseen mechanical destruction, VELUX flat
2.7 Environment and health during manufacturing
roof windows must be replaced; apart from potential injuries
All factories are ISO 14001 and ISO 45001 certified.
from glass cullet, no adverse effects on human health or the
2.8 Product processing/Installation environment are to be expected.
The product is delivered to the customer in two parts, a top and
2.14 Re-use phase
bottom part. After the hole in the roof is prepared, the bottom
VELUX flat roof windows can be dismantled manually without
part of the product can be installed with the use of a
any problems. The metal parts are usually recycled, and the
screwdriver, after which the top unit can be fastened to the
plastic parts and wood are sent for thermal recycling for energy
bottom unit.
recovery. Flat glass can be recycled whereas laminated glass is
2.9 Packaging usually used as secondary aggregate in road construction or
landfilling.
The packaging usually consists of:
- polyethylene film
2.15 Disposal
- polystyrene foam parts
VELUX flat roof windows are mostly inert and can be disposed
- cardboard
of in an appropriate landfill. However, due to the value of the
materials or the carbon content of the plastic parts and wood,
The use of other packaging materials is possible, but
recycling or energy recovery is preferable and common.
insignificant in terms of quantity.
Waste code according to the European Waste List (Regulation
The plastic packaging (polyethylene (PE) film, polystyrene foam
on the European Waste List):
parts) can be recycled if separated by type; alternatively, they
can be incinerated.
16 02 14 electronic parts
2.10 Condition of use 17 02 01 wood
17 02 02 glass
The material composition of VELUX flat roof windows does not
17 02 03 plastics
change over their service life.
17 04 14 mixed metals
2.11 Environment and health during use
2.16 Further information
VELUX flat roof windows do not contain any pollutants that
Further documentation on the products, technical data sheets,
could be released during use.
BIM files, etc. can be found at:
www.velux.com
Environmental protection: According to current knowledge,
3. LCA: Calculation rules
1.20 m x 1.20 m = 1.44 m2.
3.1 Declared Unit
Declared unit
The declared unit is 1 piece of a solar-powered VELUX flat roof
window CVU with a base unit made of a polyurethane, heat-
treated wood and plywood with an integrated glazing unit with
3 Environmental Product Declaration - VELUX A/S - VELUX flat roof window CVU - solar-powered
Name Value Unit
3.3 Estimates and assumptions
Declared unit 1 pce.
No further assumptions and estimates relevant to the result had
Area 1.44 m²
to be made beyond the points made in this chapter 3 and in
Weight 134 kg chapter 4.
3.4 Cut-off criteria
3.2 System boundary No data available from the company survey was neglected.
Type of EPD: Cradle to gate with options, with modules C1 – These include, among other things, material use, energy
C4, and module D (A1-A3, C1-C3, D and additional modules demand (heat, electricity), packaging materials of raw materials
(insofar as they are generated as waste) and product
The production of VELUX flat roof windows (modules A1-A3) packaging, consumables in production, waste treatment and
includes raw material extraction, energy generation, waste the transport of all inputs and outputs.
treatment and all transports up to the factory gate. In With this approach, mass and energy flows below 1 % were
accordance with COUNCIL REGULATION (EU) No 333/2011, also accounted for. No processes were neglected that would
secondary metals are modeled as part of the product system have been known to the project managers and would have
from the moment they are available as unmixed scrap. contributed significantly to the indicators of the impact
Waste or secondary fuels are not used for production. assessment.
3.5 Background data
Module A4 is not declared due to large variances in transport
Ecoinvent 3.8 (2021) is used as the background database.
distances between the production site and the construction site,
where the product is installed. 3.6 Data quality
The foreground data are based on extensive and detailed data
Module A5: The products are delivered to the construction site
collection at the production site. The foreground data could be
ready to be installed. Manual installation is assumed, and
fully linked with corresponding data records from the
electricity consumption related to electric drilling machines,
background database ecoinvent 3.8.
screw drivers, etc. is considered to be negligible. The
The background data was updated in 2021. Thus, the quality of
combustible packaging material (plastics, wood, etc.) is
the foreground and background data can be rated as very
assumed to be thermally treated in a municipal waste
good.
incineration plant with an efficiency R1 < 0.6 (according to the
ecoinvent dataset used); the recovered energy is declared as 3.7 Period under review
exported energy. Metals and cardboard are recycled; it is The LCA data represents the production conditions for the year
assumed that these fractions reach the end-of-waste state after 2021.
having been sorted and transported (as a conservative choice)
to a recycler. No packaging waste is landfilled. 3.8 Geographic Representativeness
Land or region, in which the declared product system is
Modules B1 to B7 are not relevant for the product under manufactured, used or handled at the end of the product´s
consideration or no significant environmental impacts occur. lifespan: Europe
Module C1 includes manual dismantling, with no significant
environmental impact. 3.9 Allocation
No co-products are generated during the production of the
Module C2 comprises the transport of the dismantled VELUX VELUX products. Sorted production scrap of the different
flat roof window to a sorting plant and then to a waste metals, notably aluminium, is considered a secondary material
incineration plant for the thermally treated plastic fraction. with no economic value (so no burdens allocated) and
considered in the quantification of net flows leaving the product
Modules C3/C4: given the complexity of the inventoried system. This approach is chosen to ensure a coherent
products, a mixed end-of-life scenario is modelled, allowing the quantification of net flows entering module D.
different materials to follow their most likely path. Biogenic carbon is allocated based on physical flows
As a rule of thumb, metals are recycled and plastics are regardless of the allocation procedure chosen for the process.
incinerated (also due to the very limited data availability of The biogenic carbon content of wood products entering or
plastics recycling and its benefits); coated and uncoated flat leaving the product system is quantified (manually) as part of
glass is assumed to be recycled whereas laminated glass is the GWP in conformity with DIN EN 16485.
assumed to be landfilled due to very limited recycling potential.
Metals and flat glass recycled; it is assumed that these fractions No processes were modelled as part of the foreground model
reach the end-of-waste state after having been sorted and that would have required an allocation of multi-input processes.
transported to a recycler; laminated glass is landfilled. The Background datasets on municipal waste incineration plants
combustible material (plastics, wood, etc.) is assumed to be were taken from ecoinvent without any modification.
thermally treated in a municipal waste incineration plant.
Allocation of reuse, recycling and recovery was avoided by the
Module D includes the benefits and burdens associated with cut-off approach in the foreground model in line with DIN EN
recycling metals beyond the system boundary, resulting from 15804.
the treatment of recycled materials from the point of end-of-
3.10 Comparability
waste to the point of substitution (as loads) and substitution of
primary resources (as benefits). Basically, a comparison or an evaluation of EPD data is only
It also includes the benefits and burdens associated with possible if all the data sets to be compared were created
energy recovery from plastic waste in a municipal waste according to EN 15804 and the building context, respectively
incineration plant, as modeled in Module C3. the product-specific characteristics of performance, are taken
In Module D, only net flows of metals leaving the product into account.
system are considered.
4 Environmental Product Declaration - VELUX A/S - VELUX flat roof window CVU - solar-powered
4. LCA: Scenarios and additional technical information
Name Value Unit
Characteristic product properties of biogenic carbon
Reference service life
according to
30 a
Information on describing the biogenic carbon content at manufacturer's
factury gate declaration
Name ValueUnit The product has passed
Declared product
kg internal quality controls and
Biogenic carbon content in product 4.57 properties (at the gate) -
C complies with EAD 220062-00-
and finishes
0401 for CE marking
Biogenic carbon content in accompanying kg
2.24
packaging C Design application
parameters (if instructed
Note: 1 kg of biogenic carbon is equivalent to 44/12 kg of CO .
2 by the manufacturer), Installation according to
including the references assembly instructions and -
to the appropriate state of the art.
practices and application
codes
An assumed quality of
Module A5
work, when installed in
The products are delivered to the construction site ready to be Carried out in accordance with
accordance with the -
installed. Manual installation is assumed, and electricity the manufacturer's instructions.
manufacturer’s
consumption related to electric drilling machines, screw drivers,
instructions
etc. is considered to be negligible.
Outdoor environment, (for The declared products are
The combustible packaging material (plastics, wood, etc.) is
outdoor applications), e.g. intended for installation outside
assumed to be transported 50 km with a lorry 16-32 metric
weathering, pollutants, UVthe building: They are therefore
tons, EURO6 to an incineration plant with an efficiency R1 < 0.6 -
and wind exposure, designed to withstand outdoor
(according to the ecoinvent dataset used); the recovered
building orientation, conditions throughout their
energy is declared as exported energy; for its quantification an
shading, temperature service life.
efficiency of 25.6 % is assumed for the production of heat and
13.0 % for the production of electricity (always referring to the Indoor environment (for
The declared products are not
lower heating value of the waste). indoor applications), e.g.
intended for installation inside -
Metals and cardboard are recycled; it is assumed that these temperature, moisture,
a building.
fractions reach the end-of-waste state after having been sorted chemical exposure
and transported (as a conservative choice) to a recycler over Usage conditions, e.g. Standard use in any type of
150 km with a lorry 16-32 metric tons, EURO6. frequency of use, building, i.e. opening/closing -
No packaging waste is landfilled. mechanical exposure as often as necessary.
The use of multi-way pallets is not taken into account as The declared products are
packaging material. designed for a reference life of
Maintenance e.g. required
30 years, with the motor
frequency, type and
Reference service life replaced every 15 years. They -
quality and replacement
are maintained by cleaning
of components
water at the discretion of the
building occupants.
Module B1
The products are assumed to have no direct emissions during
the use phase. The indicator values of Module B1 are thus 0.
For biogenic carbon stored in product, see above.
Module B2
The maintenance scenario (B2) covers the replacement of the
motor over the service life of the product. Given that the
detailed composition of the motor and its electronic
components is not known, potential loads and benefits related
to the motor and electronics are disregarded.
Annual cleaning with water (e.g., using 1 l/m2 of tap water per
annual cleaning) is neglected.
Module B6
For motor-operated flat roof windows, electricity is used both in
stand-by and during operations.
Module C1
Manual de-installation is assumed, electricity consumption
related to electric screw drivers, etc. is considered to be
negligible. Thus, no environmental impacts are declared in
5 Environmental Product Declaration - VELUX A/S - VELUX flat roof window CVU - solar-powered
module C1. with an efficiency R1 < 0.6 (according to the ecoinvent dataset
used); 25.57 % of the lower heating value of the plastic parts
Module C2 are recovered as heat and 13.0 % as electricity. Recovered
Given the complexity of the inventoried products, a mixed end- energy is reported as 'exported energy' and considered in
of-life scenario is modelled, allowing the different materials to Module D.
follow their most likely path.
Some of the material, notably laminated flat glass is assumed
It should also be noted that the deconstruction and waste to be landfilled.
treatment scenario can vary a lot, depending on the actual
situation. Thus, a generic end-of-life scenario is assumed. Module D
Module D contains the benefits and loads beyond the system
As a rule of thumb, metals are recycled, plastics are incinerated boundary related to the recycling of metals, which result from
(also due to the very limited availability on plastics recycling the treatment of recycled materials from the point of end-of-
and its benefits); coated and uncoated flat glass is assumed to waste status to the point of substitution (as loads) and the
be recycled whereas laminated glass is assumed to be substitution of primary resources (as benefits).
landfilled due to very limited recycling potential.
Furthermore, it includes the benefits of raw material substitution
The combustible material (plastics, wood, etc.) is assumed to of the recycling of flat glass, with the exception of laminated
be transported 50 km with a lorry 16-32 metric tons, EURO6 to glass, which cannot be used for the production of glass again.
an incineration plant. Recovered flat glass is assumed to have reached the end-of-
waste state as sorted glass cullet; glass cullet is assumed to
Metals and flat glass recycled; it is assumed that these fractions replace virgin raw material for glass production – impacts on
reach the end-of-waste state after having been sorted and the energy required to remelt recycled glass as compared to
transported to a recycler over 150 km with a lorry 16-32 metric virgin glass production are neglected due to a lack of data.
tons, EURO6.
It also includes the benefits and loads related to the energy
Laminated glass is landfilled, including a transport of 30 km with recovery from plastic wastes in a MWIP as modelled in
a lorry 16-32 metric tons, EURO6. Modules A3, A5 and C3.
Module C3 The benefits of the recycling of the motor and electronic parts
A consumption of 0.03 kWh/kg of electricity for shredding and are not considered due to the absence of data on its
sorting and 0.437 MJ/kg of diesel fuel for internal logistics are composition and recycled content.
taken into account to disassemble the product. The recovered
material leaves the product system as 'materials for recycling'. Due to a lack of data for plastics from de-construction activities,
The net amounts of the metals leaving the product system are the substitution potential of recycled plastics is not taken into
considered as 'use of secondary material' in Module D. account.
Module C4 Only net flows leaving the product system are considered in
As stated above, it is assumed that 100 % of the plastic parts module D.
and the wooden parts are treated in a waste incineration plant
6 Environmental Product Declaration - VELUX A/S - VELUX flat roof window CVU - solar-powered
5. LCA: Results
Disclaimer:
EP-freshwater: This indicator has been calculated as 'kg P eq' as required in the characterization model (EUTREND model, Struijs et
al., 2009b, as implemented in ReCiPe; http://eplca.jrc.ec.europa.eu/LCDN/developerEF.xhtml)
DESCRIPTION OF THE SYSTEM BOUNDARY (X = INCLUDED IN LCA; MND = MODULE OR INDICATOR NOT DECLARED; MNR
= MODULE NOT RELEVANT)
Benefits and
Construction loads beyond
Product stage Use stage End of life stage
process stage the system
boundaries
la ire ta m w a Ry lp p u s tro p s n a rT g n iru tc a fu n a M e h t m o rf tro p s n a rTe tis e h t o t e ta g y lb m e s s A e s U e c n a n e tn ia M ria p e R tn e m e c a lp e R tn e m h s ib ru fe R y g re n e la n o ita re p Oe s u re ta w la n o ita re p Oe s u n o itc u rts n o c -e Dn o itilo m e d tro p s n a rT g n is s e c o rp e ts a W la s o p s iD -e s u e R-y re v o c e R-g n ilc y c e Rla itn e to p
A1 A2 A3 A4 A5 B1 B2 B3 B4 B5 B6 B7 C1 C2 C3 C4 D
X X X MND X X X MNR MNR MNR X MND X X X X X
RESULTS OF THE LCA - ENVIRONMENTAL IMPACT according to EN 15804+A2: 1 piece VELUX flat roof window CVU - solar-
powered, 1.20 m x 1.20 m = 1.44 m2
Parameter Unit A1-A3 A5 B1 B2 B6 C1 C2 C3 C4 D
GWP-total kg CO 2 eq 4.55E+02 2.14E+01 0 3.21E+01 0 0 1.35E+00 3.11E+00 6.45E+01 -1.93E+02
GWP-fossil kg CO 2 eq 4.87E+02 5.33E+00 0 3.21E+01 0 0 1.34E+00 3.03E+00 4.77E+01 -1.92E+02
GWP-
biogenic kg CO 2 eq -3.28E+01 1.6E+01 0 -1.39E-17 0 0 0 7.65E-02 1.67E+01 0
GWP-luluc kg CO 2 eq 6.77E-01 1.92E-04 0 4.27E-02 0 0 5.47E-04 2.01E-03 3.5E-03 -6.03E-01
ODP kg CFC11 eq 7.23E-05 1.08E-07 0 5.59E-06 0 0 3.15E-07 1.15E-07 1.31E-06 -8.08E-06
AP mol H+ eq 2.59E+00 3.09E-03 0 4.33E-01 0 0 7.63E-03 7.21E-03 4.27E-02 -1.07E+00
EP-
kg P eq 1.49E-02 3.72E-06 0 2.43E-03 0 0 9.89E-06 2.3E-04 1.06E-04 -8.86E-03
freshwater
EP-marine kg N eq 4.77E-01 1.17E-03 0 3.85E-02 0 0 2.74E-03 2.35E-03 1.86E-02 -1.62E-01
EP-terrestrial mol N eq 4.86E+00 1.29E-02 0 4.13E-01 0 0 3.02E-02 2.65E-02 1.92E-01 -1.79E+00
kg NMVOC
POCP 1.47E+00 3.63E-03 0 1.52E-01 0 0 8.62E-03 7.04E-03 4.7E-02 -5.33E-01
eq
ADPE kg Sb eq 8.98E+02 1.6E-06 0 5.48E-03 0 0 4.5E-06 3.21E-06 2.85E-05 1.22E-03
ADPF MJ 4.77E+03 7.11E+00 0 4.01E+02 0 0 2.07E+01 2.5E+01 3.99E+01 -1.95E+03
m3 world eq
WDP 1.65E+02 2.98E-02 0 3.51E+01 0 0 6.79E-02 1.35E-01 2.09E+00 -2.21E+01
deprived
GWP = Global warming potential; ODP = Depletion potential of the stratospheric ozone layer; AP = Acidification potential of land and water; EP =
Eutrophication potential; POCP = Formation potential of tropospheric ozone photochemical oxidants; ADPE = Abiotic depletion potential for non-fossil
resources; ADPF = Abiotic depletion potential for fossil resources; WDP = Water (user) deprivation potential)
RESULTS OF THE LCA - INDICATORS TO DESCRIBE RESOURCE USE according to EN 15804+A2: 1 piece VELUX flat roof
window CVU - solar-powered, 1.20 m x 1.20 m = 1.44 m2
Parameter Unit A1-A3 A5 B1 B2 B6 C1 C2 C3 C4 D
PERE MJ 4.1E+02 1.1E-01 0 8.1E+01 2.52E+04 0 2.93E-01 3.12E+00 1.82E+02 -2.3E+02
PERM MJ 3.64E+02 -1.84E+02 0 1.11E-16 0 0 0 -9.86E-01 -1.79E+02 0
PERT MJ 7.74E+02 -1.84E+02 0 8.29E+01 2.52E+04 0 2.93E-01 2.14E+00 3.18E+00 -2.3E+02
PENRE MJ 5.86E+03 6.95E+01 0 4E+02 0 0 2.07E+01 2.11E-05 5.23E+02 -1.96E+03
PENRM MJ 5.45E+02 -6.24E+01 0 0 0 0 0 0 -4.83E+02 0
PENRT MJ 6.41E+03 7.11E+00 0 4E+02 0 0 2.07E+01 2.11E-05 3.99E+01 -1.96E+03
SM kg 2.67E+01 0 0 1.4E+00 0 0 0 0 0 -3.53E-01
RSF MJ 0 0 0 0 0 0 0 0 0 0
NRSF MJ 0 0 0 0 0 0 0 0 0 0
FW m3 4.9E+00 1.56E-03 0 1.07E+00 0 0 2.26E-03 6.9E-03 7.01E-02 -1.12E+00
PERE = Use of renewable primary energy excluding renewable primary energy resources used as raw materials; PERM = Use of renewable primary
energy resources used as raw materials; PERT = Total use of renewable primary energy resources; PENRE = Use of non-renewable primary energy
excluding non-renewable primary energy resources used as raw materials; PENRM = Use of non-renewable primary energy resources used as raw
materials; PENRT = Total use of non-renewable primary energy resources; SM = Use of secondary material; RSF = Use of renewable secondary fuels;
NRSF = Use of non-renewable secondary fuels; FW = Use of net fresh water
RESULTS OF THE LCA – WASTE CATEGORIES AND OUTPUT FLOWS according to EN 15804+A2:
1 piece VELUX flat roof window CVU - solar-powered, 1.20 m x 1.20 m = 1.44 m2
Parameter Unit A1-A3 A5 B1 B2 B6 C1 C2 C3 C4 D
HWD kg 7.09E-02 1.93E-05 0 2.31E-02 0 0 5.28E-05 2.11E-05 8.06E-05 1.98E-02
NHWD kg 9.09E+01 5.39E-01 0 8.89E+00 0 0 1.39E+00 7.08E-01 5.81E+01 -4.03E+01
7 Environmental Product Declaration - VELUX A/S - VELUX flat roof window CVU - solar-powered
RWD kg 4.69E-02 1.01E-04 0 2.08E-03 0 0 2.99E-04 2.25E-04 3.27E-04 -6.67E-03
CRU kg 0 0 0 0 0 0 0 0 0 0
MFR kg 5.25E+00 1.09E+01 0 3.5E+00 0 0 0 4.56E+01 0 0
MER kg 0 0 0 0 0 0 0 0 0 0
EEE MJ 1.52E+01 8.11E+00 0 1.68E+00 0 0 0 0 8.6E+01 0
EET MJ 2.96E+01 1.6E+01 0 3.31E+00 0 0 0 0 1.69E+02 0
HWD = Hazardous waste disposed; NHWD = Non-hazardous waste disposed; RWD = Radioactive waste disposed; CRU = Components for re-use;
MFR = Materials for recycling; MER = Materials for energy recovery; EEE = Exported electrical energy; EET = Exported thermal energy
RESULTS OF THE LCA – additional impact categories according to EN 15804+A2-optional:
1 piece VELUX flat roof window CVU - solar-powered, 1.20 m x 1.20 m = 1.44 m2
Parameter Unit A1-A3 A5 B1 B2 B6 C1 C2 C3 C4 D
Disease
PM 2.3E-05 4.44E-08 0 2.03E-06 0 0 1.21E-07 1.07E-07 2.75E-07 -1.23E-05
incidence
IR kBq U235 eq 1.11E+01 3.05E-02 0 1.37E+00 0 0 8.99E-02 8.68E-02 1.52E-01 -2.57E+00
ETP-fw CTUe 1.26E+04 2.73E+01 0 2.33E+03 0 0 1.64E+01 2.2E+01 5.04E+02 -3.44E+03
HTP-c CTUh 1.21E-06 9.25E-10 0 1.14E-07 0 0 6.54E-10 4.95E-10 1.58E-08 -1.71E-07
HTP-nc CTUh 1.7E-05 1.24E-08 0 3.59E-06 0 0 1.89E-08 2.93E-08 1.81E-07 -2.53E-06
SQP SQP 2.35E+03 5.98E+00 0 1.69E+02 0 0 1.77E+01 3.63E+00 2.73E+01 -2.52E+02
PM = Potential incidence of disease due to PM emissions; IR = Potential Human exposure efficiency relative to U235; ETP-fw = Potential comparative
Toxic Unit for ecosystems; HTP-c = Potential comparative Toxic Unit for humans (cancerogenic); HTP-nc = Potential comparative Toxic Unit for humans
(not cancerogenic); SQP = Potential soil quality index
Disclaimer 1 – for the indicator 'Potential Human exposure efficiency relative to U235'.This impact category deals mainly with the
eventual impact of low dose ionizing radiation on human health of the nuclear fuel cycle. It does not consider effects due to possible
nuclear accidents, occupational exposure or radioactive waste disposal in underground facilities. Potential ionizing radiation from the
soil, radon and from some construction materials is also not measured by this indicator.
Disclaimer 2 – for the indicators 'abiotic depletion potential for non-fossil resources', 'abiotic depletion potential for fossil resources',
'water (user) deprivation potential, deprivation-weighted water consumption', 'potential comparative toxic unit for ecosystems', 'potential
comparative toxic unit for humans – cancerogenic', 'Potential comparative toxic unit for humans - not cancerogenic', 'potential soil
quality index'. The results of this environmental impact indicator shall be used with care as the uncertainties on these results are high
as there is limited experience with the indicator.
6. LCA: Interpretation
Figure 1 illustrates the relative contributions of the different
modules along the life cycle of the declared products.
one impact category to another.
Benefits and burdens beyond the system boundary (module D)
Figure 1: Relative environmental impacts of the different are in the order of 0% to almost 100% of the impacts over the
life cycle stages for the solar-powered flat roof window product life cycle (modules A1-C4). [1] The use of renewable
CVU primary energy is mainly caused by the use of operational
energy, thus the use stage is the main drivers of this impact
The largest part of environmental impacts is caused during category; for the use of non-renewable primary energy, the
production (modules A1-A3) ranging from 80% to roughly production stage (modules A1-A3) is the most impacting life
100%, and during the generation of operational energy (module cycle stage.
B2) The relative contributions of these main drivers differs from Material use of primary energy is negligible and related to
8 Environmental Product Declaration - VELUX A/S - VELUX flat roof window CVU - solar-powered
plastic parts of the product and packaging material. The wastes are mainly caused by the European electricity mix.
material use of primary energy is transferred to its energy use
when the materials containing primary energy are incinerated [1] Benefits resulting from the recycling of plastics as well as
with energy recovery. from the recycling of the electronic parts are disregarded due to
Non-hazardous waste as the quantitatively most relevant waste the lack of data on the recycling processes and related to the
flows is mainly caused during the production of the glass and detailed composition of the electronic parts.
during disposal of the product; hazardous and radio-active
7. Requisite evidence
to AltholzVO
7.1 Formaldehyde Not applicable; not tested based on applicable product
Not tested based on applicable product standard. standard. 7.4. Fire gas toxicity
Not tested based on applicable product standard. 7.5 VOC
7.2 MDI emissions
Not tested based on applicable product standard. 7.3 Not tested based on applicable product standard.
Checking of pre-treatment of substances used according
8. References
Product category rules of IBU methods.
IBU (2021) EAD 220062-00-0401
IBU (2021): General Instructions for the EPD Programme of the EAD 220062-00-0401, June 2017, rooflight with bonded or
Institut Bauen & Umwelt e.V. (General Instructions for the IBU mechanically fastened cover glass
EPD Programme). Version 2.0, Institut Bauen & Umwelt, Berlin
EN 16485
IBU (2017) DIN EN 16485:2014-07, Round and sawn timber -
IBU (2017): PCR Teil A: PCR Part A: Calculation rules for the Environmental Product Declarations - Product category rules
life cycle assessment and requirements for the project report. for wood and wood-based products for use in construction;
Version 1.8., Institut Bauen & Umwelt, Berlin. German version EN 16485:2014.
IBU (2021) ECHA-List
IBU (2021):PCR Part B: Requirements on the EPD for windows The Candidate List of substances of very high concern,
and doors. Version 2021/01, Institut Bauen & Umwelt, Berlin. available via https://echa.europa.eu/nl/-/four-newsubstances-
added-to-the-candidate-list.
Standards and legal documents
Regulation on biocidal products
EN 15804 REGULATION (EU) No 528/2012 OF THE EUROPEAN
DIN EN 15804+A2:2019, Sustainability of construction works - PARLIAMENT AND OF THE COUNCIL of 22 May 2012
Environmental product declarations - Core rules for the product concerning the making available on the market and use of
category construction products. biocidal products.
ISO 14025 Regulation (EU) Nr. 305/2011(CPR)
DIN EN ISO 14025:2006-07, Environmental labels and REGULATION (EU) No 305/2011 OF THE EUROPEAN
declarations - Type III Environmental declarations - Principles PARLIAMENT AND OF THE COUNCIL of 9 March 2011 laying
and procedures. down harmonised conditions for the marketing of construction
products and repealing Council Directive 89/106/EEC.
ISO 14044
DIN EN ISO 14044:2006-07, Environmental management - Life COUNCIL REGULATION (EU) No 333/2011
cycle assessment - Requirements and guidance (ISO COUNCIL REGULATION (EU) No 333/2011 of 31 March 2011
14044:2006); German and English versions EN ISO establishing criteria determining when certain types of scrap
14044:2006. metal cease to be waste under Directive 2008/98/EC of the
European Parliament and of the Council.
ISO 9001
DIN EN ISO 9001:2015, Quality management systems - European Waste List (Waste index)
Requirements. http://www.gesetze-im-internet.de/avv/anlage.htm
ISO 14001 Additional references
DIN EN ISO 14001:2015: Environmental management
systems - Requirements with guidance for use. Weidema et al. (2013)
Weidema, B., C. Bauer, R. Hischier, C. Mutel, T. Nemecek, J.
ISO 45001 Reinhard, C.O. Vadenbo, G. Wernet (2013): Overview and
ISO 45001:2018-03, Occupational health and safety methodology, Data quality guideline for the ecoinvent database
management systems - Requirements with guidance for use. version 3. ecoinvent report no. 1 (v3), St. Gallen, Schweiz.
EN 1873 ecoinvent 3.8
DIN EN 1873:2005, Prefabricated accessories for roofing - ecoinvent 3.8, LCA database, 12/2021. Ecoinvent centre,
Individual rooflights of plastics - Product specification and test Zürich.
9 Environmental Product Declaration - VELUX A/S - VELUX flat roof window CVU - solar-powered
Publisher
Institut Bauen und Umwelt e.V. +49 (0)30 3087748- 0
Hegelplatz 1 info@ibu-epd.com
10117 Berlin www.ibu-epd.com
Germany
Programme holder
Institut Bauen und Umwelt e.V. +49 (0)30 3087748- 0
Hegelplatz 1 info@ibu-epd.com
10117 Berlin www.ibu-epd.com
Germany
Author of the Life Cycle Assessment
Dr. Frank Werner - Umwelt & Entwicklung + 41 (0)44 241 39 06
Kammelenbergstrasse 30 frank@frankwerner.ch
9011 St. Gallen http://www.frankwerner.ch/
Switzerland
Owner of the Declaration
VELUX Group +4545164726
Ådalsvej 99 jakob.roerbech@velux.com
2970 Hørsholm www.velux.com
Denmark
10 Environmental Product Declaration - VELUX A/S - VELUX flat roof window CVU - solar-powered
