ENVIRONMENTAL PRODUCT DECLARATION
as per ISO 14025 and EN 15804+A2
Owner of the Declaration Hilti Aktiengesellschaft
Publisher Institut Bauen und Umwelt e.V. (IBU)
Programme holder Institut Bauen und Umwelt e.V. (IBU)
Declaration number EPD-HIL-20240159-CBJ1-EN
Issue date 19/07/2024
Valid to 18/07/2029
MFT-FOX HT & MFT-FOX VT
Hilti AG
www.ibu-epd.com | https://epd-online.com
General Information
Hilti AG MFT-FOX HT & MFT-FOX VT
Programme holder Owner of the declaration
IBU – Institut Bauen und Umwelt e.V. Hilti Aktiengesellschaft
Hegelplatz 1 Feldkircher Strasse 100
10117 Berlin 9494 Schaan
Germany Liechtenstein
Declaration number Declared product / declared unit
EPD-HIL-20240159-CBJ1-EN The declared product is the MFT-FOX HT 320 L 11 as a
representative product for the FOX T portfolio. The declared unit is to kg of
product. The packaging is also included in the calculation.
This declaration is based on the product category rules: Scope:
Building metals, 01/08/2021 This document relates to the MFT-FOX HT 320 L 11 as a representative
(PCR checked and approved by the SVR) product for the MFT-FOX T portfolio including FOX VT and FOX HT. FOX T
products cover the same applications and are equal in material constitution
and have been summarized in this EPD.
Issue date FOX HT and FOX VT can be divided into two classes with 1 bracket size.
FOX VT to be used for the vertical façade application, FOX HT for
19/07/2024
horizontal ones. Moreover, FOX HT 320 L 11 is chosen because it displays
the highest weight of this product group, leading to the most conservative
results.
Valid to
The owner of the declaration shall be liable for the underlying information
18/07/2029 and evidence; the IBU shall not be liable with respect to manufacturer
information, life cycle assessment data and evidences.
The EPD was created according to the specifications of EN 15804+A2. In
the following, the standard will be simplified as EN 15804.
Verification
The standard EN 15804 serves as the core PCR
Independent verification of the declaration and data according to ISO
14025:2011
internally X externally
Dipl.-Ing. Hans Peters
(Chairman of Institut Bauen und Umwelt e.V.)
Florian Pronold Matthias Klingler,
(Managing Director Institut Bauen und Umwelt e.V.) (Independent verifier)
1 Environmental Product Declaration - Hilti AG - MFT-FOX HT & MFT-FOX VT
Product
Product description/Product definition Application
MFT-FOX T is designed as an aluminium substructure system. MFT-FOX T items are developed to be fixed on base materials
The brackets are suitable for all façade cladding. The products like concrete, masonry, steel frame structure and
are used for fastening ventilated façade substructure to wood. This product is used as a substructure for
concrete, masonry, steel frame structure and wood. They ventilated façade (rainscreen) applications.
enable mounting façade substructures on the primary structure According to the method of installation to the base
as a helping hand bracket and can be used to install vertical material – anchors, screws or direct fastening can be
and horizontal support rails. used – with different hole geometries in the base plate.
During the application the horizontal profiles are connected
For the placing on the market of the product in the European to the brackets with specially designed screws, which combine
Union/European Free Trade Association (EU/EFTA) (with the the fix and flexible point in one connection point.
exception of Switzerland) Regulation (EU) No. 305/2011 (CPR) Due to thermal expansion of the profile, the brackets take over
applies. The product needs a declaration of performance taking this movement. With this system, wall tolerances of
into consideration EN 1090-1:2009+A1:2011. up to 40 mm can be balanced.
Technical Data
Technical documentation according to EN 1090-3.
Constructional data
Name Value Unit
Thickness Baseplate 4 mm
Length 140 - 320 mm
Length Steps 20 mm
Height 80 / 150 mm
Width 62 mm
Performance data of the product in accordance with
the declaration of performance with respect to its
essential characteristics according to EN 1090-
1:2009+A1:2011 Standard for execution of steel
structures and aluminium structures. The structural
parts made of aluminum correspond to following
harmonized standards: EN 1090-1, DIN EN 1999-1-1 +
DIN EN 1993-1-4 incl. national annexes, DIN 18516-1.
The product has a CE-marking Hilti MFT EN 1090.
Base materials/Ancillary materials
The raw material used for the production of this
product is aluminium alloy according to the
standard EN AW-6063-T66 with 200g (63% of product
weight). The alloy is a widely used extrusion alloy,
suitable for various applications. The material used for
the plastic part is fiberglass-reinforced plastic (polyamid)
with 180g (37% of product weight).
This product ontains substances listed in the candidate list
(date
05.04.2022) exceeding 0.1 percentage by mass: no
This product contains other carcinogenic, mutagenic, reprotoxic
(CMR) substances in categories 1A or 1B which
are not on the candidate list, exceeding 0.1 percentage by
mass: no
Biocide products were added to this construction
product or it has been treated with biocide products
(this then concerns a treated product as defined by the
(EU) Ordinance on Biocide Products No. 528/2012): no
Packaging
The packaging of this product is carton. This cardboard
packaging can be recycled.
Reference service life
The MFT-FOX T systems have a minimum service life
of 35 years when used as prescribed according to the
BBA Certificate (British Board of Agreement). However,
the actual service life can be considerably longer.
2 Environmental Product Declaration - Hilti AG - MFT-FOX HT & MFT-FOX VT
LCA: Calculation rules
The primary products are sourced from the European Union
Declared Unit and Asia. Transport is by lorry and ship. The following flow
The declared product here is an aluminium profile from HILTI charts illustrate the underlying production process.
AG with the designation MFT-FOX HT 320 L11 as a
representative product from the MFT-FOX HT & MFT-FOX VT
portfolio. It is the heaviest product with the additional screw in
the portfolio. The declared unit refers to 1 kg of aluminium
profile. The packaging, based on 1 kg of aluminium profile, is
also included in the calculation at 0.031 kg. The following table
shows the data of the declared unit.
Declared unit and mass reference
Name Value Unit
Declared unit 1 kg
Figure Information modules A 1 to A3 of the product.
Gross density 2700 kg/m3
System boundary
Type of EPD: Cradle to factory gate with modules C1-C4 and D.
The following information modules are defined as system
boundaries in this study:
Figure Information modules A 1 to A3 of the packaging.
Production stage (A1- A3):
- A1, raw material extraction, In the information modules C1 to C4, the deconstruction or
- A2, transport to the manufacturer, demolition from the building, the transport to waste disposal,
- A3, production. the waste treatment and disposal of the product are recorded.
Furthermore, reuse, recovery and recycling potentials are
End of life (C1- C4): reported in information module D.
- C1, dismantling/demolition,
Geographic Representativeness
- C2, transport,
Land or region, in which the declared product system is
- C3, waste treatment,
manufactured, used or handled at the end of the product´s
- C4, disposal.
lifespan: Global
Reuse, recovery and recycling potential (D)
Comparability
In order to accurately record the indicators and environmental
Basically, a comparison or an evaluation of EPD data is only
impacts of the declared unit, a total of 8 information modules
possible if all the data sets to be compared were created
are considered. The information modules A1 to A3 describe the
according to EN 15804 and the building context, respectively
provision of materials, transport to the production site and the
the product-specific characteristics of performance, are taken
production processes of the product itself.
into account. The database referred to in this study is LCA for
Experts by Sphera. (V1 2023)
LCA: Scenarios and additional technical information
declared unit. The electricity consumption is calculated using a
Characteristic product properties of biogenic carbon European electricity mix.
The declared product does not contain any biogenic
Name Value Unit
Carbon.Note: 1kg of of biogenic carbon is equivalent to
Collected as mixed construction waste 1 kg
44/12 kg of CO2
Recycling 0.5285 kg
Information on describing the biogenic carbon content at
Energy recovery 0.444 kg
factory gate
Name Value Unit Reuse, recovery and/or recycling potentials (D), relevant
Biogenic carbon content in accompanying kg scenario information
0.000337
packaging C In Module D, the metallic components are added to the primer
material data sets through a recycling scenario of 85% and the
plastic components are thermally utilised, thereby generating
thermal and electrical energy.
End of life (C1 - C4)
Name Value Unit
The demolition of the installation system from the building is
Stainless Steel 0,018 kg
calculated in information module C1. The demolition is carried
out using an electric screwdriver. The electrical energy Aluminium 0,427 kg
consumption for the tool is assumed to be 0.5 MJ for the
3 Environmental Product Declaration - Hilti AG - MFT-FOX HT & MFT-FOX VT
LCA: Results
DESCRIPTION OF THE SYSTEM BOUNDARY (X = INCLUDED IN LCA; MND = MODULE OR INDICATOR NOT DECLARED; MNR
= MODULE NOT RELEVANT)
Benefits and
Construction loads beyond
Product stage Use stage End of life stage
process stage the system
boundaries
la ire ta m w a Ry lp p u s tro p s n a rT g n iru tc a fu n a M e h t m o rf tro p s n a rTe tis e h t o t e ta g y lb m e s s A e s U e c n a n e tn ia M ria p e R tn e m e c a lp e R tn e m h s ib ru fe R y g re n e la n o ita re p Oe s u re ta w la n o ita re p Oe s u n o itc u rts n o c -e Dn o itilo m e d tro p s n a rT g n is s e c o rp e ts a W la s o p s iD -e s u e R-y re v o c e R-g n ilc y c e Rla itn e to p
A1 A2 A3 A4 A5 B1 B2 B3 B4 B5 B6 B7 C1 C2 C3 C4 D
X X X MND MND MND MND MNR MNR MNR MND MND X X X X X
RESULTS OF THE LCA - ENVIRONMENTAL IMPACT according to EN 15804+A2: 1 kg MFT-FOX HT320 L11
Parameter Unit A1-A3 C1 C2 C3 C4 D
Global Warming Potential total (GWP-total) kg CO 2 eq 6.57E+00 5.88E-02 7.39E-03 1.39E+00 0 -4.55E+00
Global Warming Potential fossil fuels (GWP-fossil) kg CO 2 eq 6.57E+00 5.87E-02 7.42E-03 1.39E+00 0 -4.55E+00
Global Warming Potential biogenic (GWP-biogenic) kg CO 2 eq 2.27E-03 2.92E-05 0 2.36E-05 0 -1.5E-03
Global Warming Potential luluc (GWP-luluc) kg CO 2 eq 1.96E-03 5.37E-06 6.79E-05 2.06E-05 0 -1.07E-03
Depletion potential of the stratospheric ozone layer (ODP) kg CFC11 eq 9.21E-12 5.77E-13 6.42E-16 7.01E-14 0 -8.62E-12
Acidification potential of land and water (AP) mol H+ eq 2.42E-02 8.94E-05 8.82E-06 1.51E-04 0 -1.86E-02
Eutrophication potential aquatic freshwater (EP-freshwater) kg P eq 4.46E-06 5.8E-08 2.67E-08 2.43E-08 0 -2.62E-06
Eutrophication potential aquatic marine (EP-marine) kg N eq 3.89E-03 2.52E-05 2.99E-06 3.49E-05 0 -2.83E-03
Eutrophication potential terrestrial (EP-terrestrial) mol N eq 4.23E-02 2.66E-04 3.62E-05 7.14E-04 0 -3.08E-02
Formation potential of tropospheric ozone photochemical oxidants kg NMVOC
1.21E-02 6.97E-05 7.57E-06 1.02E-04 0 -8.53E-03
(POCP) eq
Abiotic depletion potential for non fossil resources (ADPE) kg Sb eq 5.13E-06 2.84E-09 4.73E-10 3.35E-09 0 -4.17E-06
Abiotic depletion potential for fossil resources (ADPF) MJ 1.09E+02 1.29E+00 9.97E-02 2.16E-01 0 -6.45E+00
m3 world eq
Water use (WDP) 7.63E-01 4.93E-03 8.45E-05 1.29E-01 0 -6.07E-01
deprived
RESULTS OF THE LCA - INDICATORS TO DESCRIBE RESOURCE USE according to EN 15804+A2: 1 kg MFT-FOX HT320 L11
Parameter Unit A1-A3 C1 C2 C3 C4 D
Renewable primary energy as energy carrier (PERE) MJ 2.86E+01 1.77E-01 7.05E-03 4.68E-02 0 -2.36E+01
Renewable primary energy resources as material utilization
MJ 4.7E-01 0 0 0 0 0
(PERM)
Total use of renewable primary energy resources (PERT) MJ 2.91E+01 1.77E-01 7.05E-03 4.68E-02 0 -2.36E+01
Non renewable primary energy as energy carrier (PENRE) MJ 8.91E+01 1.29E+00 9.99E-02 1.99E+01 0 -6.46E+01
Non renewable primary energy as material utilization (PENRM) MJ 1.97E+01 0 0 -1.97E+01 0 0
Total use of non renewable primary energy resources (PENRT) MJ 1.09E+02 1.29E+00 9.99E-02 2.16E-01 0 -6.46E+01
Use of secondary material (SM) kg 0 0 0 0 0 0
Use of renewable secondary fuels (RSF) MJ 0 0 0 0 0 0
Use of non renewable secondary fuels (NRSF) MJ 0 0 0 0 0 0
Use of net fresh water (FW) m3 7.01E-02 2.96E-04 7.77E-06 3.02E-03 -5.52E-02 -5.52E-02
RESULTS OF THE LCA – WASTE CATEGORIES AND OUTPUT FLOWS according to EN 15804+A2:
1 kg MFT-FOX HT320 L11
Parameter Unit A1-A3 C1 C2 C3 C4 D
Hazardous waste disposed (HWD) kg 9.59E-09 7.48E-11 3.7E-13 3.59E-12 0 -4.69E-09
Non hazardous waste disposed (NHWD) kg 1.32E+00 2.84E-04 1.44E-05 5.53E-03 0 -1.08E+00
Radioactive waste disposed (RWD) kg 4.01E-03 2.01E-04 1.29E-07 1.06E-05 0 -4.31E-03
Components for re-use (CRU) kg 0 0 0 0 0 0
Materials for recycling (MFR) kg 2.89E-01 0 0 0 0 0
Materials for energy recovery (MER) kg 0 0 0 0 0 0
Exported electrical energy (EEE) MJ 0 0 0 2.97E+00 0 0
Exported thermal energy (EET) MJ 0 0 0 5.28E+00 0 0
RESULTS OF THE LCA – additional impact categories according to EN 15804+A2-optional:
1 kg MFT-FOX HT320 L11
Parameter Unit A1-A3 C1 C2 C3 C4 D
Disease
Incidence of disease due to PM emissions (PM) ND ND ND ND ND ND
incidence
Human exposure efficiency relative to U235 (IR) kBq U235 eq ND ND ND ND ND ND
Comparative toxic unit for ecosystems (ETP-fw) CTUe ND ND ND ND ND ND
Comparative toxic unit for humans (carcinogenic) (HTP-c) CTUh ND ND ND ND ND ND
Comparative toxic unit for humans (noncarcinogenic) (HTP-nc) CTUh ND ND ND ND ND ND
4 Environmental Product Declaration - Hilti AG - MFT-FOX HT & MFT-FOX VT
Soil quality index (SQP) SQP ND ND ND ND ND ND
Disclaimer 1 – for the indicator “Potential Human exposure efficiency relative to U235”. This impact category deals mainly with the
eventual impact of low-dose ionizing radiation on human health of the nuclear fuel cycle. It does not consider effects due to possible
nuclear accidents, occupational exposure or radioactive waste disposal in underground facilities. Potential ionizing radiation from the
soil, radon and from some construction materials is also not measured by this indicator.
Disclaimer 2 – for the indicators “abiotic depletion potential for non-fossil resources”, “abiotic depletion potential for fossil resources”,
“water (user) deprivation potential, deprivation-weighted water consumption”, “potential comparative toxic unit for ecosystems”,
“potential comparative toxic unit for humans – cancerogenic”, “Potential comparative toxic unit for humans - not cancerogenic”,
“potential soil quality index”. The results of this environmental impact indicator shall be used with care as the uncertainties on these
results are high as there is limited experience with the indicator.
References
DIN EN 1090-1
Standard for execution of steel structures and aluminium BBA Certificate (British Board of Agreement)
structures The British Board of Agreement is a UK body issuing
certificates
DIN EN 1999-1-1 + DIN EN 1993-1-4 for construction products and systems and providing inspection
Eurocode 9: Design of aluminum structures - Part 1-4: General services in support of their designers and installers.
design rules
Calculation rules: PCR - Part A
DIN 18516-1 Product category rules for construction products and services -
DIN 18516-1:2010-06 Cladding for external walls, ventilated at Calculation rules for the eco-balance and requirements for the
rear facades – Part 1: Requirements, princicples of testing background report V1.3, Institut Bauen und Umwelt e.V.,
08.2022.
EN 1090-1:2009+A1:2011
Standard for execution of steel structures and aluminium CML 2001 April. 2015
structures Indicators for environmental impacts, Leiden: Universität
EN AW-6063-T66 Leiden,
Type of aluminium alloy http://cml.leiden.edu/software/datacmlia.
html#downloads (20.08.2022)
EN 15804
EN 15804:2012+A2:2019+AC:2021, Sustainability IBU 2021
ofconstruction works — Environmental Product Declarations — General Instructions for the EPD programme of Institut Bauen
Core rules for the product category of construction products. und Umwelt e.V. Version 2.0,
Berlin: Institut Bauen und Umwelt e.V., 2021
ISO 14025 www.ibu-epd.de
DIN EN /ISO 14025:2011-10/, Environmental labels and
declarations — Type III environmental Product category rules for construction products – Part B
declarations — Principles and procedures Institut Bauen und Umwelt e.V, Berlin (pub.): Product Category
Rules for Construction Products from the range
Regulation (EU) No. 305/2011 ofEnvironmental Product Declarations for Institut Bauen und
Construction Product Regulation (CPR) Umwelt (IBU), PConstruction metals ,.01.08.2021
Regulation (EC) No 1907/2006
REACH Regulation Sphera
LCA for Experts: Ganzheitliche Bilanzierung Leinfelden-
Regulation (EU) No 528/2012 Echterdingen; Sphera Solution GmbH (Hrsg.)
on EU Biocidal Products www.gabi-software.com/deutsch/index/
(27.06.2023)
Other references
5 Environmental Product Declaration - Hilti AG - MFT-FOX HT & MFT-FOX VT
Publisher
Institut Bauen und Umwelt e.V. +49 (0)30 3087748- 0
Hegelplatz 1 info@ibu-epd.com
10117 Berlin www.ibu-epd.com
Germany
Programme holder
Institut Bauen und Umwelt e.V. +49 (0)30 3087748- 0
Hegelplatz 1 info@ibu-epd.com
10117 Berlin www.ibu-epd.com
Germany
Author of the Life Cycle Assessment
FIT-Umwelttechnik GmbH 05362 72 69 474
Westerstr. 13 bertram@fit-umwelttechnik.de
38442 Wolfsburg www.fit-umwelttechnik.com
Germany
Owner of the Declaration
Hilti Aktiengesellschaft +423 234 2111
Feldkircher Strasse 100 HAGHSE@hilti.com
9494 Schaan www.hilti.com
Liechtenstein
6 Environmental Product Declaration - Hilti AG - MFT-FOX HT & MFT-FOX VT
