ENVIRONMENTAL PRODUCT DECLARATION
as per ISO 14025 and EN 15804+A2
Owner of the Declaration dormakaba International Holding GmbH
Publisher Institut Bauen und Umwelt e.V. (IBU)
Programme holder Institut Bauen und Umwelt e.V. (IBU)
Declaration number EPD-DOR-20210284-CBA1-EN
Issue date 26.11.2021
Valid to 25.11.2026
Terminal 97 00
dormakaba
www.ibu-epd.com | https://epd-online.com
General Information
dormakaba Terminal 97 00
Programme holder Owner of the declaration
IBU – Institut Bauen und Umwelt e.V. dormakaba International Holding GmbH
Hegelplatz 1 DORMA Platz 1
10117 Berlin 58256 Ennepetal
Germany Germany
Declaration number Declared product / declared unit
EPD-DOR-20210284-CBA1-EN 1 piece of the product: Terminal 97 00
This declaration is based on the product category rules: Scope:
Electronic and physical Access Control Systems, 01.08.2021 This EPD refers to a specific product manufactured by dormakaba. The
(PCR checked and approved by the SVR) production site is located in Villingen-Schwenningen (Germany).
The data represents the year 2019.
Issue date The owner of the declaration shall be liable for the underlying information
and evidence; the IBU shall not be liable with respect to manufacturer
26.11.2021
information, life cycle assessment data and evidences.
The EPD was created according to the specifications of EN 15804+A2. In
Valid to
the following, the standard will be simplified as EN 15804.
25.11.2026
Verification
The standard EN 15804 serves as the core PCR
Independent verification of the declaration and data according to ISO
14025:2011
internally X externally
Dipl.-Ing. Hans Peters
(Chairman of Institut Bauen und Umwelt e.V.)
Florian Pronold Dr.-Ing. Wolfram Trinius,
(Managing Director Institut Bauen und Umwelt e.V.) (Independent verifier)
1 Environmental Product Declaration - dormakaba - Terminal 97 00
Product
• USB 2.0, RS232
Product description/Product definition
Versatile, multi-functional and customizable: the terminal 97 00 Power supply
is a multi-purpose device. With its modular upgradability it • PoE IEEE802.3at, Power class 0/4
represents modern, easy and secure attendance recording as • 24V DC
well as intelligent access management and targeted staff • 100-240V AC 50/60 Hz
communication. Even multimedia contents like training films • UPS (optional)
and staff info can be integrated easily. The user identification is
done via integrated Radio-Frequency Identification (RFID) Installation
reader using an RFID medium or smartphone. A biometric • Wall mounting
fingerprint reader and swipe readers are optional. For the • Class of protection: IP20/IP54
placing on the market in the European Union/European Free
Trade Association (EU/EFTA) (with the exception of The product is not harmonised in accordance with the
Switzerland) the following legal provisions apply: Construction Product Regulations (CPR) but in accordance with
• Electromagnetic Compatibility Directive (EMC) other provisions for harmonisation of the EU. Compliance with
• Low Voltage Directive (LVD) the European Union Directive and technical specifications:
• Radio Equipment Directive (RED) • EN 62368-1:2014
• Restriction of Hazardous Substances (RoHS) • EN 55032:2015
• EN 50581:2012 • EN 55024:2010 + A1:2015
The CE-marking takes into account the proof of conformity with • EN 61000-3-2:2014
the respective harmonized standards based on the legal • EN 61000-3-3:2013
provisions above. For the application and use the respective • EN 62471:2008
national provisions apply. • EN 60529:1991 + A1:2000 + A2:2013
• EN 301489-1 V1.9.2
Application
• EN 301489-3 V1.6.1
• Attendance recording • EN 300330 V2.1.1
• Door Control • EN 50364:2010
• Staff Communication • EN 300328 V2.1.1
• EN 62311:2008
Technical Data The product is subject to CE marking according to the relevant
The Terminal 97 00 has the following technical properties: harmonization legislation.
Name Value Unit
Operating Temperature -5 - 45 °C In addition, the product also conforms to the following
standards:
Operating Humidity 5 - 85 %
• UL 62368-1:2014
Width Dimension 264 mm
• CAN/CSA-22.2 No. 62368-1:2014
Height Dimension 207 mm
• FCC Part 15 Class C
Depth Dimension 96 mm
Weight (without packaging) 1,5 kg Base materials/Ancillary materials
Weight (with packaging) 2,1 kg The major material compositions including the packaging of the
product are listed below:
Power consumption "on mode" 10 W
Name Value Unit
Power consumption "idle mode" 8 W
Paper 31 %
Power consumption "standby mode" 5 W
Glass 26 %
Host Interface
Plastics 26 %
• Ethernet 10/100/1000BASE-T IEEE802.3 compatible
• Optional WLAN IEEE802.11 a/b/g/n (2,4/5 GHz) Electronics 15 %
Aluminium 1 %
User Interface Others <1 %
• 7' illuminated touch display
The product includes partial articles which contain substances
• Loudspeaker, Microphone
listed in the Candidate List
• Camera (optional)
of REACH Regulation 1907/2006/EC (date: 08.07.2021)
• RFID reader
exceeding 0.1 percentage by mass: yes
- MRD (LEGIC / MIFARE)
- HID (iClass SE Prox) • Lead (Pb): 7439-92-1 (CAS-No.) is included in some of
• Biometric fingerprint reader the alloys used. The concentration of lead in each
• MAG stripe/ barcode reader individual alloy does not exceed 4.0% (by mass).
• Booking via smartphone
- NFC (Android) The Candidate List can be found on the ECHA website
- BLE (Android+iOS) address: https:echa.europa.eu/de/home.
• CardLink to integrate offline door components
Reference service life
The reference service life of the dormakaba Terminal 97 00 is
Peripherals Interface estimated to be 10 years. This number is based on the support
• 4 digital inputs / 2 relay outputs and service life and is not an estimated lifetime.
2 Environmental Product Declaration - dormakaba - Terminal 97 00
LCA: Calculation rules
Declared Unit Use stage - Module B6
The declared unit is 1 piece of the product: Terminal 97 00. The use stage related to the operation of the building includes:
Declared unit — B6, operational energy use
Name Value Unit
End-of-life stage– Modules C1-C4 and D
Declared unit 1 pce.
The end-of-life stage includes:
Conversion factor to 1 kg (kg per declared unit) 0.476 - — C1, de-construction, demolition:
Product weight including packaging 2,1 kg — C2, transport to waste processing;
— C3, waste processing for reuse, recovery and/or recycling;
System boundary — C4, disposal;
including provision and all transport, provision of all materials,
The type of EPD is: cradle to gate with options, modules C1–
products and related energy and water use.
C4, and module D (A1–A3 + C + D and additional modules: A4
+ A5 + B6)
Module D (Benefits and loads beyond the system boundary)
includes:
Production - Module A1-A3
— D, recycling potentials, expressed as net impacts and
The product stage includes:
benefits.
— A1, raw material extraction, processing and mechanical
treatments, processing of secondary material input (e.g.
Geographic Representativeness
recycling processes),
Land or region, in which the declared product system is
— A2, transport to the manufacturer,
manufactured, used or handled at the end of the product´s
— A3, manufacturing and assembly
lifespan: Germany
including provision of all materials, products and energy, as well
as waste processing up to the end-of waste state.
Comparability
Construction stage - Modules A4-A5
Basically, a comparison or an evaluation of EPD data is only
The construction process stage includes:
possible if all the data sets to be compared were created
— A4, transport to the building site;
according to EN 15804 and the building context, respectively
— A5, installation into the building;
the product-specific characteristics of performance, are taken
including provision of all materials, products and energy, as well
into account. Background database: GaBi, SP40.
as waste processing up to the end-of-waste state or disposal of
final residues during the construction process stage.
LCA: Scenarios and additional technical information
Operational energy use (B6)
Characteristic product properties of biogenic carbon
Name Value Unit
Information on describing the biogenic Carbon Content at
Energy consumption for 1 year 48,9 kWh
factory gate
Power consumption "on mode" 10 W
Name ValueUnit
Hours per day in use in "on mode" 1 h
kg
Biogenic carbon content in product 0.02 C Power consumption "idle mode" 8 W
Biogenic carbon content in accompanying kg Hours per day in use in "idle mode" 3 h
0.22
packaging C Power consumption "standy mode" 5 W
Hours per day in use in "standby mode" 20 h
Note: 1 kg of biogenic carbon is equivalent to 44/12 kg of CO .
2
Days per year in use 365 days
Two scenarios are declared:
The following technical scenario information is required for the
declared modules. - B6 is calculated with US and EU electricity grid mix according
Transport to the building site (A4) to dormakaba's market
- B6/1 is calculated with EU-28 electricity grid mix
Name Value Unit
Litres of fuel per 1 kg (truck) 0.00276 l/100km
End of life (C1-C4)
Transport distance (truck) 1620 km
C1: The product dismantling from the building is done manually
Capacity utilisation (including empty runs) 51 %
without environmental burden.
Transport distance (ship) 5000 km
Name Value Unit
Installation into the building (A5) Collected separately waste type waste type 1.5 kg
Name Value Unit Recycling 0.336 kg
Waste Packaging (paper) 0,6 kg Energy recovery 0.558 kg
Final deposition 0,606 kg
Reference service life
Transportation to Waste Processing Site 50 km
Name Value Unit
Life Span according to the manufacturer 10 a
3 Environmental Product Declaration - dormakaba - Terminal 97 00
Region for end of life: Global Reuse, recovery and/or recycling potentials (D), relevant
scenario information
Collection rate is 100%.
4 Environmental Product Declaration - dormakaba - Terminal 97 00
LCA: Results
B6 declares the environmental impact for the use stage (B6: region US/EU and B6/1: region EU).
DESCRIPTION OF THE SYSTEM BOUNDARY (X = INCLUDED IN LCA; MND = MODULE OR INDICATOR NOT DECLARED; MNR
= MODULE NOT RELEVANT)
Benefits and
Construction loads beyond
Product stage Use stage End of life stage
process stage the system
boundaries
la ire ta m w a Ry lp p u s tro p s n a rT g n iru tc a fu n a M e h t m o rf tro p s n a rTe tis e h t o t e ta g y lb m e s s A e s U e c n a n e tn ia M ria p e R tn e m e c a lp e R tn e m h s ib ru fe R y g re n e la n o ita re p Oe s u re ta w la n o ita re p Oe s u n o itc u rts n o c -e Dn o itilo m e d tro p s n a rT g n is s e c o rp e ts a W la s o p s iD -e s u e R-y re v o c e R-g n ilc y c e Rla itn e to p
A1 A2 A3 A4 A5 B1 B2 B3 B4 B5 B6 B7 C1 C2 C3 C4 D
X X X X X MND MND MNR MNR MNR X MND X X X X X
RESULTS OF THE LCA - ENVIRONMENTAL IMPACT according to EN 15804+A2: 1 piece Terminal 97 00
Parameter Unit A1-A3 A4 A5 B6 B6/1 C1 C2 C3 C4 D
GWP-total kg CO 2 eq 6.02E+01 3.32E-01 8.51E-01 2.29E+02 1.98E+02 0 7E-03 1.42E+00 9E-03 -1.03E+01
GWP-fossil kg CO 2 eq 6.1E+01 3.19E-01 2.1E-02 2.28E+02 1.97E+02 0 6E-03 1.42E+00 9E-03 -1.02E+01
GWP-
biogenic kg CO 2 eq -7.85E-01 1.3E-02 8.29E-01 4.17E-01 6.56E-01 0 2.92E-04 3.31E-05 3.14E-05 -1.6E-02
GWP-luluc kg CO 2 eq 5.4E-02 7.48E-06 1.4E-05 2.04E-01 2.85E-01 0 1.5E-07 8.02E-05 2.65E-05 -4E-03
ODP kg CFC11 eq 3.68E-09 3.33E-17 1.53E-16 2.99E-12 4.33E-12 0 6.66E-19 7.16E-16 3.41E-17 -1.3E-12
AP mol H+ eq 4.08E-01 2E-03 2.38E-04 4.39E-01 4.35E-01 0 6.31E-06 2.53E-04 6.59E-05 -1.47E-01
EP-
kg P eq 2.36E-04 6.86E-08 3E-08 3.76E-04 5.26E-04 0 1.35E-09 1.14E-07 1.58E-08 -3.23E-06
freshwater
EP-marine kg N eq 6.05E-02 4.25E-04 8.6E-05 9.6E-02 9.65E-02 0 2.01E-06 5.7E-05 1.7E-05 -1.7E-02
EP-terrestrial mol N eq 6.46E-01 5E-03 1E-03 1.02E+00 1.01E+00 0 2.23E-05 1E-03 1.87E-04 -1.9E-01
kg NMVOC
POCP 1.79E-01 1E-03 2.28E-04 2.67E-01 2.64E-01 0 5.68E-06 1.58E-04 5.14E-05 -5.3E-02
eq
ADPE kg Sb eq 8E-03 9.41E-09 2.42E-09 5.6E-05 5.7E-05 0 1.89E-10 9.82E-09 8.25E-10 -7E-03
ADPF MJ 8.43E+02 4.45E+00 2.69E-01 3.85E+03 3.46E+03 0 8.9E-02 6.58E-01 1.21E-01 -1.14E+02
m3 world eq
WDP 1.06E+01 6.19E-04 1.05E-01 4.7E+01 4.29E+01 0 1.24E-05 1.45E-01 9.63E-04 -1.62E+00
deprived
GWP = Global warming potential; ODP = Depletion potential of the stratospheric ozone layer; AP = Acidification potential of land and water; EP =
Eutrophication potential; POCP = Formation potential of tropospheric ozone photochemical oxidants; ADPE = Abiotic depletion potential for non-fossil
resources; ADPF = Abiotic depletion potential for fossil resources; WDP = Water (user) deprivation potential)
RESULTS OF THE LCA - INDICATORS TO DESCRIBE RESOURCE USE according to EN 15804+A2: 1 piece Terminal 97 00
Parameter Unit A1-A3 A4 A5 B6 B6/1 C1 C2 C3 C4 D
PERE MJ 1.22E+02 1.4E-02 7.25E+00 1.2E+03 1.53E+03 0 2.82E-04 8.07E-01 1.6E-02 -1.13E+01
PERM MJ 7.84E+00 0 -7.2E+00 0 0 0 0 -6.36E-01 0 0
PERT MJ 1.3E+02 1.4E-02 4.9E-02 1.2E+03 1.53E+03 0 2.82E-04 1.71E-01 1.6E-02 -1.13E+01
PENRE MJ 8.25E+02 4.45E+00 2.69E-01 3.86E+03 3.46E+03 0 9E-02 2.42E+01 1.21E-01 -1.14E+02
PENRM MJ 2.36E+01 0 0 0 0 0 0 -2.36E+01 0 0
PENRT MJ 8.49E+02 4.45E+00 2.69E-01 3.86E+03 3.46E+03 0 9E-02 6.58E-01 1.21E-01 -1.14E+02
SM kg 9.24E-05 0 0 0 0 0 0 0 0 0
RSF MJ 0 0 0 0 0 0 0 0 0 0
NRSF MJ 0 0 0 0 0 0 0 0 0 0
FW m3 3.14E-01 2.53E-05 2E-03 1.72E+00 1.77E+00 0 5.06E-07 3E-03 3.04E-05 -4.3E-02
PERE = Use of renewable primary energy excluding renewable primary energy resources used as raw materials; PERM = Use of renewable primary
energy resources used as raw materials; PERT = Total use of renewable primary energy resources; PENRE = Use of non-renewable primary energy
excluding non-renewable primary energy resources used as raw materials; PENRM = Use of non-renewable primary energy resources used as raw
materials; PENRT = Total use of non-renewable primary energy resources; SM = Use of secondary material; RSF = Use of renewable secondary fuels;
NRSF = Use of non-renewable secondary fuels; FW = Use of net fresh water
RESULTS OF THE LCA – WASTE CATEGORIES AND OUTPUT FLOWS according to EN 15804+A2:
1 piece Terminal 97 00
Parameter Unit A1-A3 A4 A5 B6 B6/1 C1 C2 C3 C4 D
HWD kg 2.94E-05 4.32E-10 3.96E-10 1.54E-06 1.43E-06 0 8.68E-12 2.51E-09 1.84E-09 -1.37E-07
NHWD kg 1.46E+00 4.55E-04 2.7E-02 2.03E+00 2.46E+00 0 9.15E-06 1.47E-01 6.06E-01 -3.68E-01
RWD kg 3.12E-02 4.8E-06 1.41E-05 4.74E-01 5.25E-01 0 9.61E-08 2.44E-05 1.37E-06 -3E-03
CRU kg 0 0 0 0 0 0 0 0 0 0
MFR kg 0 0 0 0 0 0 0 3.45E-01 0 0
MER kg 0 0 0 0 0 0 0 0 0 0
EEE MJ 1.07E-01 0 1.29E+00 0 0 0 0 0 0 0
5 Environmental Product Declaration - dormakaba - Terminal 97 00
EET MJ 1.95E-01 0 2.33E+00 0 0 0 0 0 0 0
HWD = Hazardous waste disposed; NHWD = Non-hazardous waste disposed; RWD = Radioactive waste disposed; CRU = Components for re-use;
MFR = Materials for recycling; MER = Materials for energy recovery; EEE = Exported electrical energy; EET = Exported thermal energy
RESULTS OF THE LCA – additional impact categories according to EN 15804+A2-optional:
1 piece Terminal 97 00
Parameter Unit A1-A3 A4 A5 B6 B6/1 C1 C2 C3 C4 D
Disease
PM 4.01E-06 2.31E-08 1.32E-09 3.78E-06 3.65E-06 0 3.32E-11 3.22E-09 8.16E-10 -1.23E-06
incidence
IR kBq U235 eq 3E+00 6.86E-04 2E-03 6.48E+01 8.62E+01 0 1.37E-05 2E-03 1.41E-04 -3.4E-01
ETP-fw CTUe 4.83E+02 3.15E+00 1.27E-01 1.42E+03 1.48E-03 0 6.3E-02 2.47E-01 6.9E-02 -2.55E+01
HTP-c CTUh 1.73E-08 5.93E-11 6.74E-12 3.59E-08 4.09E-08 0 1.19E-12 2.14E-11 1.02E-11 -1.76E-09
HTP-nc CTUh 1.02E-06 2.56E-09 2.92E-10 1.34E-06 1.51E-06 0 5.1E-11 2.16E-09 1.13E-09 -9.73E-08
SQP SQP 3.01E+02 1.1E-02 7.1E-02 8.24E+02 1.1E+03 0 2.3E-04 1.97E-01 2.5E-02 -1.29E+01
PM = Potential incidence of disease due to PM emissions; IR = Potential Human exposure efficiency relative to U235; ETP-fw = Potential comparative
Toxic Unit for ecosystems; HTP-c = Potential comparative Toxic Unit for humans (cancerogenic); HTP-nc = Potential comparative Toxic Unit for humans
(not cancerogenic); SQP = Potential soil quality index
Disclaimer 1 – for the indicator IRP
This impact category deals mainly with the eventual impact of low dose ionizing radiation on human health of the nuclear fuel cycle. It
does not consider effects due to possible nuclear accidents, occupational exposure nor due to radioactive waste disposal in
underground facilities. Potential ionizing radiation from the soil, from radon and from some construction materials is also not measured
by this indicator.
Disclaimer 2 – for the indicators ADPE, ADPF, WDP, ETP-fw, HTP-c, HTP-nc, SQP
The results of this environmental impact indicator shall be used with care as the uncertainties on these results are high or as there is
limited experience with the indicator.
References
Standards EN 50581
EN 50581:2012, Technical documentation for the assessment
CAN/CSA-22.2 No. 62368-1 of electrical and electronic products with respect to the
CAN/CSA-22.2 No. 62368-1:2014, Audio/video, information and restriction of hazardous substances.
communication technologyequipment — Part 1: Safety
requirements. EN 55024+A1
EN 55024:2010+A1:2015, Information technology equipment -
EN 15804+A2 Immunity characteristics - Limits and methods of measurement.
EN 15804:2019+A2 (in press), Sustainability of construction
works — Environmental Product Declarations — Core rules for EN 55032
the product category of construction products. EN 55032:2015, Electromagnetic compatibility of multimedia
equipment - Emission Requirements.
EN 300328 V2.1.1
EN 300328 V2.1.1, Wideband transmission systems - Data EN 60529+A1+A2
transmission equipment operating in the 2,4 GHz ISM band and EN 60529:1991 + A1:2000 +A2:2013, Degrees of protection
using wide band modulation techniques - Harmonised Standard provided by enclosures (IP 20).
covering the essential requirements of article 3.2 of the
Directive 2014/53/EU. EN 61000-3-2
EN 61000-3-2:2014, Electromagnetic compatibility (EMC) - Part
EN 300330 3-2: Limits - Limits for harmonic current emissions (equipment
EN 300330 V2.1.1, Short Range Devices (SRD) - Radio input current ≤ 16 A per phase).
equipment in the frequency range 9 kHz to 25 MHz and
inductive loop systems in the frequency range 9 kHz to 30 EN 61000-3-3
MHz - Harmonised Standard covering the essential EN 61000-3-3:2013, Electromagnetic compatibility (EMC) - Part
requirements of article 3.2 of the Directive 2014/53/EU. 3-3: Limits - Limitation of voltage changes, voltage fluctuations
and flicker in public low-voltage supply systems, for equipment
EN 301489-1 V1.9.2 + V1.6.1 with rated current ≤ 16 A per phase and not subject to
EN 301489-1 V1.9.2 + V1.6.1, ElectroMagnetic Compatibility conditional connection.
(EMC) standard for radio equipment and services - Part 1:
Common technical requirements - Harmonised Standard EN 62311
covering the essential requirements of article 3.1(b) of Directive EN 62311:2008, Assessment of electronic and electrical
2014/53/EU and the essential requirements of article 6 of equipment related to human exposure restrictions for
Directive 2014/30/EU. electromagnetic fields.
EN 50364 EN 62368-1
EN 50364:2010; Limitation of human exposure to EN 62368-1:2014, Audio/video, information and communication
electromagnetic fields from devices operating in the frequency technology equipment - Part 1: Safety requirements.
range 0 Hz to 300 GHz, used in Electronic Article Surveillance
(EAS), Radio Frequency Identification (RFID) and similar EN 62471
applications. EN 62471:2008, Photobiological safety of lamps and lamp
systems.
6 Environmental Product Declaration - dormakaba - Terminal 97 00
UL 62368-1
Electromagnetic Compatibility Directive (EMC) UL 62368-1:2014, Standard for Audio/video, information and
Directive 2014/30/EU of the European Parliamant and of the communication technology equipment - Part 1: Safety
Council of 26 February 2014 on the harmonisation of the laws requirements.
of the Member States relating to electromagnetic compatibility.
Further References
FCC 47 CFR Part 15: FCC Part 15
The FCC 47 CFR Part 15 from the Federal Communications IBU 2021
Commission: rules and regulations for EMC. Institut Bauen und Umwelt e.V.: General Instructions for the
EPDs programme of Institut Bauen und Umwelt e.V. Version
ISO 14025 2.0., Berlin: Institut Bauen und Umwelt e.V., 2021. www.ibu-
DIN EN ISO 14025:2011-10, Environmental labels and epd.com
declarations — Type III environmental declarations — GaBi ts software
Principles and procedures. Sphera Solutions GmbH
Gabi Software System and Database for Life Cycle Engineering
Low Voltage Directive (LVD) 1992-2020 Version 10.0.0.71 University of Stuttgart Leinfelden-
Directive 2014/35/EU of the European Parliament and of the Echterdingen
Council of 26 February 2014 on the harmonisation of the laws
of the Member States relating to the making available on the GaBi ts documentation
market of electrical equipment designed for use within certain GaBi life cycle inventory data documentation (https://www.gabi-
voltage limits. software.com/support/gabi/gabi-database-2020-lci-
documentation/).
Radio Equipment Directive (RED)
Directive 2014/53/EU of the European Parliament and of the LCA-tool dormakaba
Council of 16 April 2014 on the harmonisation of the laws of the LCA tool, version 1.0.
Member States relating to the making available on the market Developed by Sphera Solutions GmbH.
of radio equipment and repealing Directive 1999/5/EC.
PCR Part A
REACH Regulation 1907/2006/EC PCR – Part A:
Regulation (EC) No 1907/2006 of the European Parliament and Calculation Rules for the Life Cycle As-sessment and
of the Council on the Registration, Evaluation, Authorisation Requirements on the Project Re-port according to EN
and Restriction of Chemicals (REACH). 15804+A2:2019, Version 1.0, Institut Bauen und Umwelt e.V.,
www.ibu-epd.com.
Restriction of Hazardous Substances (RoHS)
Directive on the restriction of the use of certain hazardous PCR Part B
substances in electrical and electronic equipment (RoHS), PCR – Part B: Requirements on the EPD for Building Hardware
Directive (EU) No 2011/65. product, version 1.2, Institut Bauen und Umwelt e.V., www.ibu-
epd.com, 2017.
7 Environmental Product Declaration - dormakaba - Terminal 97 00
Publisher
Institut Bauen und Umwelt e.V. +49 (0)30 3087748- 0
Hegelplatz 1 info@ibu-epd.com
10117 Berlin www.ibu-epd.com
Germany
Programme holder
Institut Bauen und Umwelt e.V. +49 (0)30 3087748- 0
Hegelplatz 1 info@ibu-epd.com
10117 Berlin www.ibu-epd.com
Germany
Author of the Life Cycle Assessment
Sphera Solutions GmbH +49 711 341817-0
Hauptstraße 111- 113 info@sphera.com
70771 Leinfelden-Echterdingen www.sphera.com
Germany
Owner of the Declaration
dormakaba International Holding GmbH +49 2333 793-0
DORMA Platz 1 info.de@dormakaba.com
58256 Ennepetal www.dormakaba.com
Germany
8 Environmental Product Declaration - dormakaba - Terminal 97 00
