ENVIRONMENTAL PRODUCT DECLARATION
as per ISO 14025 and EN 15804+A2
Owner of the Declaration Kima Accessories Aps
Publisher Institut Bauen und Umwelt e.V. (IBU)
Programme holder Institut Bauen und Umwelt e.V. (IBU)
Declaration number EPD-KIM-20230120-CBC1-EN
Issue date 06.06.2023
Valid to 05.06.2028
Plastic products made of recycled PP or ABS
Kima Accessories Aps
www.ibu-epd.com | https://epd-online.com
General Information
Kima Accessories Aps Plastic products made of recycled PP or ABS
Programme holder Owner of the declaration
IBU – Institut Bauen und Umwelt e.V. Kima Accessories Aps
Hegelplatz 1 Kastanievej 3
10117 Berlin 6862 Tistrup
Germany Denmark
Declaration number Declared product / declared unit
EPD-KIM-20230120-CBC1-EN 1 kg protective building products made of recycled polypropylene (PP),
styrene-ethylene-styrene (SEBS) or acrylonitrile-butadiene-styrene (ABS)
including mounting material.
This declaration is based on the product category rules: Scope:
Boards and panels made of plastic (exterior applications), This environmental product declaration described is a representative EPD
01.08.2021 of protective building products produced at Kima Accessories facility in
(PCR checked and approved by the SVR) Tistrup, Denmark.
It includes the following products:
• Eaves filler combs
Issue date
• Fixing bracket for eaves filler comb
06.06.2023 • KimaAir inside and outside vent
• Underlay pipes
• Underlay tightener
Valid to • Brick wall valve
• Moisture protector
05.06.2028
• Rebate protector
• Insulation disc
• Iso-pipe
• Adapter for iso-pipe
• Hip trays
All of the above-mentioned products are made of recycled PP, SEBS or
ABS and through either injection moulding or extrusion. The data is based
on data collected at the production site and data delivered by suppliers.
The data represents the production of the period 01.07.2021 to
30.06.2022.
The owner of the declaration shall be liable for the underlying information
and evidence; the IBU shall not be liable with respect to manufacturer
Dipl.-Ing. Hans Peters information, life cycle assessment data and evidences.
(Chairman of Institut Bauen und Umwelt e.V.)
The EPD was created according to the specifications of EN 15804+A2. In
the following, the standard will be simplified as EN 15804.
Verification
The standard EN 15804 serves as the core PCR
Independent verification of the declaration and data according to ISO
14025:2011
internally X externally
Dipl.-Ing. Hans Peters Dr.-Ing. Nikolay Minkov,
(Managing Director Institut Bauen und Umwelt e.V.) (Independent verifier)
1 Environmental Product Declaration - Kima Accessories Aps - Plastic products made of recycled PP or ABS
Product
• Adapter for iso-pipe - Used for the transition between
Product description/Product definition ice tube and the exhaust duct tube
This environmental product declaration covers several • Hip tray - Roof base plate
protective building products made of plastic by either injection • Brick wall valve - Makes ventilation and lets moisture
moulding or extrusion. The product group under study covers inside the wall out
16 products, which are all made of recycled polypropylene • Moisture protector - Prevents moisture from penetrating
(PP), styrene-ethylene-styrene (SEBS) or acrylonitrile- element walls.
butadiene-styrene (ABS). • Rebate protector - Prevents moisture from penetrating
element walls.
The product included are:
Technical Data
• R2000: Eaves filler comb 1m 0.055 kg/m
The different plastic materials PP, SEBS and ABS serving as
• R2002: Eaves filler comb 5m - 0.275 kg/pcs
input materials for the products covered by this environmental
• R2003: Eaves filler comb vented - 0.125 kg/m
product declaration are tested in accordance with the following
• R2004: Fixing bracket for eaves filler comb - 0.020
standards.
kg/pcs
• R2023: KimaAir outside/in vent - 0.077 kg/pcs
Recycled PP:
• R2005: KimaAir inside/out vent - 0.077 kg/pcs
• R2006: Underlaypipe feedthrough - 0.475 kg/pcs • ISO 1133
• R2007: Underlay tightener - 0,040 kg/pcs • ISO 179-1
• M9100: Brick wall valve with lid - 0.027 kg/pcs • ISO 180
• M9500: Brick wall valve without lid - 0.023 kg/pcs • ISO 527-1-2
• R2016: Moisture protector - 0.140 kg/pcs • ISO 1183
• R2022BL: Insulation disc - 0.008 kg/pcs • ISO 3302-1
• R2020: Iso-pipe - 0.500 kg/pcs
• R2021: Adapter for iso-pipe - 0.115 kg/pcs Recycled ABS:
• R2009: Hip tray - 0.480 kg/m
• ISO 1133
• R2040: Rebate protector - 0.250 kg/pair
• ISO 1183
Most of the products are somehow attached to the roof
• ISO 527
construction, exceptions are the brick wall valve, moisture
• ISO 178
protector and rebate protector. These products are attached to
• ISO 180-1
other parts of the building e.g., penetrating element wall etc. All
• ISO 179
the products are black and for the hip trays a small amount of
• ISO 306
masterbatch is included to ensure the black color.
• ISO 75-1
• ISO 11359
The production of Kima Accessories protective building material
• ISO 294-4
have so far not been subject to EU harmonizatoin legislation.
• ISO 1043
Hence, for the use and application of the products the
• ISO 3302-1
respective national provisions at the place of use apply.
Recycled SEBS:
Application
The products covered by this environmental product declaration • ISO 1133
have different applications. Some prevent birds, leaves and • ISO 179-1
other small animals to enter the roof space, others protect the • ISO 180
roof or other parts of the building from moisture and thereby • ISO 527-1-2
prevent the formation of mold and improve the indoor climate of • ISO 1183
the building. • ISO 3302-1
For each product, the application is listed below. Constructional data
• Eaves filler comb 1 m - Keeps roof space free from Name Value Unit
birds, leaves and large insects
Thickness 1.5 - 4.3 mm
• Eaves filler comb 5 m - Keeps roof space free from
Gross density 0.968 - 1.16 kg/m3
birds, leaves and large insects
• Eaves filler comb vented - Prevents the entry of birds Flexural strength according to ISO 178 57 MPa
and vermin into the batten cavity Melt flow rate 37-44 g/10min
• Fixing bracket for eaves filler comb - Holds ventilated Charpy impact strength 4-36 kJ/m^2
bird screen
Tensile stress 28-40 MPa
• KimaAir outside/in vent - protects roof space against
excessive condensation Performance data of the product with respect to its
• KimaAir inside/out vent - protects roof space against characteristics in accordance with the relevant technical
excessive condensation provision (no CE-marking).
• Underlay pipe feedthrough - Waterproof penetration of
Base materials/Ancillary materials
the underlay
• Underlay tightener - Ensures that the underlay stays flat,
and rainwater does not accumulate
• Insulation disc - Disc for mounting insulation
• Iso-pipe - Inside insulation of roof cap
2 Environmental Product Declaration - Kima Accessories Aps - Plastic products made of recycled PP or ABS
Name Value Unit
Reference service life
Recycled PP Main component 78 %
The reference service life is not relevant for consideration of the
Recycled SEBS Main component 12 %
LCA since the use stage modules B1-B7 are not included.
Recycled ABS Main component 8 %
Virgin PP Main component 0.1 % The expected lifetime of the products attached to the roof
Stainless steel Mounting equipment 0.2 % construction are mounted during the construction of the roof
and are typically not removed before the roof is replaced.
Polyethylene foam Mounting equipment 0.03 %
Hence, the expected lifetime is equal to the lifetime of the roof
Nylon Mounting equipment 1.3 %
which is between 20-100 years. For the products that are
Tape Mounting equipment 0.05 % integrated into other building parts such as the brick wall valve,
This product/article/at least one partial article moisture protector and rebate protector, the plastic product is
contains substances listed in the candidate list (date: integrated into the building and is typically not replaced before
10.05.2023) exceeding 0.1 percentage by mass: No the building is refurbished or demolished.
LCA: Calculation rules
state.
Declared Unit All of the above-mentioned is included in this study. Wastes and
The declared unit is 1 kg protective building products made of losses of the manufacturing processes are included in the
recycled polypropylene (PP), styrene-ethylene-styrene (SEBS) processes in which they occur according to the polluter pays
or acrylonitrile-butadiene-styrene (ABS) including mounting principle.
material.
The representative product composition of this EPD is weighted The construction of the manufacturing facility is not taken into
by the annual production volume of the period 01.07.2021 to account however, the production of spare parts for machinery is
30.06.2022. included in this study. The electricity consumption includes all
Declared unit activities at the manufacturing facility including office
equipment.
Name Value Unit
Gross density 0.97 - 1.16 kg/m3 End-of-life stage - Module C1-C4
Declared unit 1 kg The end-of-life stage includes:
Important for the products under study is, that the input material • C1, deconstruction and demolition
is recycled post-consumer plastic, which has no difference in • C2, transport to waste processing
environmental impacts compared to the respective virgin • C3, waste processing for reuse, recovery and/or
alternative. Furthermore, the manufacturing processes are recycling
mostly injection moulding (approximately 95 %) but also • C4, disposal
extrusion (approximately 5 %). The composition of input The deconstruction of the products is assumed to be done
material is calculated based on the data collected on the manually. As a result, no processes have been assigned to
amount of each product manufactured for the given time period, module C1. 95 % of the products are sold to Danish customers
which was weighted using the total production volume of the the remaining 5 % is divided between other Scandinavian
same time period. countries (4 %) and other European countries (1 %). Hence, the
transportation distance is modelled for Danish conditions. A
The robustness of the LCA values is judged to be good. The transport distance from the building to the waste processing
difference in the production processes in injection moulding and facilities of 50 km is assumed. End-of-life treatment of
extrusion is assumed to be low as the main input is electricity. packaging material is not included as module A5 is not
Here the electricity consumption was found by taking the total declared.
electricity consumption of the production facility and dividing it
by the total production volume, as it was not possible to Benefits and loads beyond the system boundaries -
measure the individual machines. The geographical Module D
representative is good, as all products are manufactured in The benefits and loads include:
Denmark.
• D, potential benefits from reuse, recycling and recovery
outside the scope of the study.
Background data is used for the modules A1, A2, module C and
• D, potential loads related to processing to reach
D. Collecting primary data in these stages will make the LCA
equivalent materials to virgin input material
stronger, however, it might not change the overall conclusion of
In this case, benefits are given to the recycling of the amount of
the LCA results.
virgin plastic and to the recycling of metal-based mounting
equipment. The loads of the regranulation of plastic as well as
System boundary
the re-melting of metal are included in this study. Furthermore,
This is a cradle-to-gate EPD with modules A1-A3, C1–C4 and
a benefit is given to the exported energy obtained from waste
D.
incineration.
Production stage - Module A1-A3 Geographic Representativeness
The production stage includes:
Land or region, in which the declared product system is
• A1, raw material extraction and processing, processing manufactured, used or handled at the end of the product´s
of secondary material from previous product systems, lifespan: Denmark
when applicable.
• A2, transport to factory gate and internal transport
Comparability
• A3, manufacturing of products and packaging, as well
as assembly and processing up to the end-of-waste
3 Environmental Product Declaration - Kima Accessories Aps - Plastic products made of recycled PP or ABS
Basically, a comparison or an evaluation of EPD data is only the product-specific characteristics of performance, are taken
possible if all the data sets to be compared were created into account. The system model EN15804 - cut-off available in
according to EN 15804 and the building context, respectively the LCI database Ecoinvent v. 3.9 is used in this EPD.
LCA: Scenarios and additional technical information
End of life (C1-C4)
Characteristic product properties of biogenic carbon
The biogenic carbon content quantifies the amount of biogenic Name Value Unit
carbon in a construction product leaving the factory gate. Both Collected separately 0.9 kg
the biogenic content of the product and the accompanying Collected as mixed construction waste 0.1 kg
packaging is declared.
Recycling Plastic mixture 0.89 kg
Recycling Stainless steel 0,002 kg
Note: 1 kg of biogenic carbon is equivalent to 44/12 kg of CO .
2
Energy recovery Plastic mixture 0.1 kg
Information on describing the biogenic Carbon Content at Reuse, recovery and/or recycling potentials (D), relevant
factory gate scenario information
Name ValueUnit The following values in the table are amounts contributing to
the loads and benefits included in module D.
kg
Biogenic carbon content in product -
C Name Value Unit
Biogenic carbon content in accompanying kg Recycling of polyethylene from module C3 0,0007 kg
0.01
packaging C Recycling of steel from module C3 0.0007 kg
Incineration of plastic mixture from module C3 0.1 kg
The following technical scenario information covers the disposal
Credits are only given to the net amount leaving the product
of the accompanying packaging material, produced in module
system that has passed the end-of-waste state.
A3, on the construction site as module A5 is not declared in this
EPD.
In the LCA calculation loads related to obtaining equivalent
Installation into the building (A5) functions as the original virgin material are included as well as
benefits of avoided production of the given virgin material.
Name Value Unit
Packaging waste for recycling (Cardboard) 0.038 kg
Packaging waste for recycling (Wood pallet) 0.025 kg
Packaging waste for incineration (Plastic film) 0.0015 kg
Packaging waste for incineration (Tape) 0.00000078 kg
4 Environmental Product Declaration - Kima Accessories Aps - Plastic products made of recycled PP or ABS
LCA: Results
The following table shows the LCA results obtained in this study.
For calculation of the results, characterization was used on a model created of individual inputs from different LCIA methods to comply
with EN15804+A2 which is yet to be fully implemented in the SimaPro software. As a result, the LCIA has been calculated in Excel
using the following methods from EcoInvent v.3.9:
• EF v.3.1 EN 15804
• EN 15804 inventory indicators according to ISO 21930
The additional indicators are retrieved by using ecoinvent cumulative LCIA results for the system model EN15804, cut-off. It follows ISO
21930 for all the datasets; hence the results include all the background processes as well as foreground processes.
C1 is declared as 0 since manual deconstruction is assumed.
C4 is declared as 0, since no landfilling is assumed in the end-of-life stage.
The estimated impact results are only relative statements which do not indicate the endpoints of the impact categories, exceeding
threshold values, safety margins or risks.
DESCRIPTION OF THE SYSTEM BOUNDARY (X = INCLUDED IN LCA; ND = MODULE OR INDICATOR NOT DECLARED; MNR =
MODULE NOT RELEVANT)
Benefits and
Construction loads beyond
Product stage Use stage End-of-life stage
process stage the system
boundaries
la ire ta m w a Ry lp p u s tro p s n a rT g n iru tc a fu n a M e h t m o rf tro p s n a rTe tis e h t o t e ta g y lb m e s s A e s U e c n a n e tn ia M ria p e R tn e m e c a lp e R tn e m h s ib ru fe R y g re n e la n o ita re p Oe s u re ta w la n o ita re p Oe s u n o itc u rts n o c -e Dn o itilo m e d tro p s n a rT g n is s e c o rp e ts a W la s o p s iD -e s u e R-y re v o c e R-g n ilc y c e Rla itn e to p
A1 A2 A3 A4 A5 B1 B2 B3 B4 B5 B6 B7 C1 C2 C3 C4 D
X X X MND MND MND MND MNR MNR MNR MND MND X X X X X
RESULTS OF THE LCA - ENVIRONMENTAL IMPACT according to EN 15804+A2: 1 kg protective building products made of
recycled polypropylene (PP), styrene-ethylene-styrene (SEBS) or acrylonitrile-butadiene-styrene (ABS) including mounting
material
Parameter Unit A1-A3 C1 C2 C3 C4 D
Global Warming Potential total (GWP-total) kg CO 2 eq 1.47E+00 0 7.32E-03 5.09E-01 0 -8.85E-03
Global Warming Potential fossil fuels (GWP-fossil) kg CO 2 eq 1.57E+00 0 7.31E-03 5.01E-01 0 -8.74E-03
Global Warming Potential biogenic (GWP-biogenic) kg CO 2 eq -9.27E-02 0 5.87E-06 7.67E-03 0 -1.02E-04
Global Warming Potential luluc (GWP-luluc) kg CO 2 eq 8.6E-04 0 3.64E-06 4.44E-04 0 -5.74E-06
Depletion potential of the stratospheric ozone layer (ODP) kg CFC11 eq 2.77E-08 0 1.62E-10 3.38E-09 0 -1.23E-10
Acidification potential of land and water (AP) mol H+ eq 5.59E-03 0 1.67E-05 7.26E-04 0 -4.24E-05
Eutrophication potential aquatic freshwater (EP-freshwater) kg P eq 5.44E-04 0 5.38E-07 1.05E-04 0 -3.13E-06
Eutrophication potential aquatic marine (EP-marine) kg N eq 1.21E-03 0 4.35E-06 2.89E-04 0 -7.97E-06
Eutrophication potential terrestrial (EP-terrestrial) mol N eq 1.19E-02 0 4.41E-05 2.2E-03 0 -8.16E-05
Formation potential of tropospheric ozone photochemical oxidants kg NMVOC
3.8E-03 0 2.64E-05 5.91E-04 0 -2.7E-05
(POCP) eq
Abiotic depletion potential for non fossil resources (ADPE) kg Sb eq 6.71E-06 0 2.39E-08 1.28E-06 0 -1.71E-07
Abiotic depletion potential for fossil resources (ADPF) MJ 2.42E+01 0 1.07E-01 2.36E+00 0 -1.15E-01
m3 world eq
Water use (WDP) 2.47E-01 0 5.48E-04 1.15E-01 0 -1.59E-03
deprived
RESULTS OF THE LCA - INDICATORS TO DESCRIBE RESOURCE USE according to EN 15804+A2: 1 kg protective building
products made of recycled polypropylene (PP), styrene-ethylene-styrene (SEBS) or acrylonitrile-butadiene-styrene (ABS)
including mounting material
Parameter Unit A1-A3 C1 C2 C3 C4 D
Renewable primary energy as energy carrier (PERE) MJ 2.42E+00 0 1.71E-03 1.89E+00 0 -1.77E-02
Renewable primary energy resources as material utilization
MJ 7.21E-01 0 0 0 0 0
(PERM)
Total use of renewable primary energy resources (PERT) MJ 3.14E+00 0 1.71E-03 1.89E+00 0 -1.77E-02
Non renewable primary energy as energy carrier (PENRE) MJ 2.36E+01 0 1.07E-01 -3.86E+01 0 -8.26E-02
Non renewable primary energy as material utilization (PENRM) MJ 6.49E-01 0 0 4.09E+01 0 -3.22E-02
Total use of non renewable primary energy resources (PENRT) MJ 2.42E+01 0 1.07E-01 2.36E+00 0 -1.15E-01
Use of secondary material (SM) kg 1.52E-02 0 4.83E-05 3.58E-03 0 -8.02E-04
Use of renewable secondary fuels (RSF) MJ 1.19E-02 0 5.91E-07 2.81E-05 0 -1.66E-06
Use of non renewable secondary fuels (NRSF) MJ 0 0 0 0 0 0
Use of net fresh water (FW) m3 2.64E-02 0 1.38E-05 4.09E-03 0 -1.03E-04
RESULTS OF THE LCA – WASTE CATEGORIES AND OUTPUT FLOWS according to EN 15804+A2:
1 kg protective building products made of recycled polypropylene (PP), styrene-ethylene-styrene (SEBS) or acrylonitrile-
butadiene-styrene (ABS) including mounting material
5 Environmental Product Declaration - Kima Accessories Aps - Plastic products made of recycled PP or ABS
Parameter Unit A1-A3 C1 C2 C3 C4 D
Hazardous waste disposed (HWD) kg 1.24E-01 0 7.26E-05 1.4E-02 0 -2.08E-03
Non hazardous waste disposed (NHWD) kg 2.62E+00 0 2.28E-03 5.9E-01 0 -1.54E-02
Radioactive waste disposed (RWD) kg 1.56E-05 0 8.94E-09 2.09E-06 0 -6.67E-08
Components for re-use (CRU) kg 0 0 0 0 0 0
Materials for recycling (MFR) kg 2.54E-02 0 8.17E-07 8.08E-01 0 -3.58E-06
Materials for energy recovery (MER) kg 8.48E-07 0 4.86E-09 3.56E-07 0 -8.85E-08
Exported electrical energy (EEE) MJ 3.82E-01 0 1.81E-05 1.85E-02 0 -1.04E-03
Exported thermal energy (EET) MJ 1.23E-02 0 4.73E-05 9.33E-04 0 -1.37E-04
RESULTS OF THE LCA – additional impact categories according to EN 15804+A2-optional:
1 kg protective building products made of recycled polypropylene (PP), styrene-ethylene-styrene (SEBS) or acrylonitrile-
butadiene-styrene (ABS) including mounting material
Parameter Unit A1-A3 C1 C2 C3 C4 D
Disease
Incidence of disease due to PM emissions (PM) 3.59E-08 0 5.92E-10 1E-08 0 -4.98E-10
incidence
Human exposure efficiency relative to U235 (IR) kBq U235 eq 3.07E-01 0 1.5E-04 4.6E-02 0 -1.13E-03
Comparative toxic unit for ecosystems (ETP-fw) CTUe 3.95E+00 0 5.22E-02 1.3E+00 0 -3.04E-02
Comparative toxic unit for humans (carcinogenic) (HTP-c) CTUh 1.19E-09 0 3.46E-12 2.85E-10 0 -1.21E-10
Comparative toxic unit for humans (noncarcinogenic) (HTP-nc) CTUh 1.92E-08 0 7.57E-11 3.58E-09 0 -1.62E-10
Soil quality index (SQP) SQP 1.51E+01 0 8E-02 3.4E+00 0 -4.06E-02
Disclaimer 1 – for the indicator 'Potential Human exposure efficiency relative to U235'.This impact category deals mainly with the
eventual impact of low-dose ionizing radiation on human health of the nuclear fuel cycle. It does not consider effects due to possible
nuclear accidents, occupational exposure or radioactive waste disposal in underground facilities. Potential ionizing radiation from the
soil, radon and from some construction materials is also not measured by this indicator.
Disclaimer 2 – for the indicators 'abiotic depletion potential for non-fossil resources', 'abiotic depletion potential for fossil resources',
'water (user) deprivation potential, deprivation-weighted water consumption', 'potential comparative toxic unit for ecosystems', 'potential
comparative toxic unit for humans – cancerogenic', 'Potential comparative toxic unit for humans - not cancerogenic', 'potential soil
quality index'. The results of this environmental impact indicator shall be used with care as the uncertainties on these results are high
as there is limited experience with the indicator.
References
Standards Determination of the melt mass-flow rate and melt volume-flow
EN 15804 rate of
EN 15804:2012+A2:2019+AC:2021, Sustainability of thermoplastics
construction works — Environmental Product Declarations —
Core rules for the product category of construction products. ISO 1183
ISO 1183:2019, Plastics – Methods for
ISO 75-1:2020 determining the density of non-cellular plastics
ISO 75-1, Plastics – Determination
of temperature of deflection under load ISO 3302-1
ISO 3302-1:2014, Classes and Tolerances
ISO 178 for Products Moulded in Solid Rubber
ISO 178:2019, Plastics – Determination
of flexural properties ISO 11359
ISO 11359:2021, Plastics –
ISO 179-1 Thermomechanical analysis
ISO 179-1:2010, Plastics – Determination
of Charpy impact properties ISO 14025
— Part 1: Non-instrumented impact test EN ISO 14025:2011, Environmental labels and declarations —
Type III environmental declarations — Principles and
ISO 180-1 procedures.
ISO 180-1:2019, Plastics — Determination of Izod impact
strength ISO 14040
ISO 14040:2006, Environmental management –Life cycle
ISO 306 assessment - Principles and framework;English version
ISO 306:2004, Plastics –
Thermoplastics materials- Determination of Vicat softening ISO 14044
temperature ISO 14044:2006, Environment Management – LifeCycle
Assessment – Requirements and Instructions;English version
ISO 527-1-2 EN ISO 14044:2006.
ISO 527-1-2:2012,
Plastics — Determination of tensile properties — Part 1: Further references
General principles
ECHA candidate list
ISO 1133 Candidate List of substances of very high concern for
ISO 1133:2011, Plastics – Authorisation
6 Environmental Product Declaration - Kima Accessories Aps - Plastic products made of recycled PP or ABS
https://echa.europa.eu/candidate-list-table [Accessed 25-05- IBU 2021
2023]. Product Category Rules for Building-Related Products
and Services, Part A: Calculation Rules for the Life
EcoInvent 3.9 Cycle Assessment and Requirements on the Project
EcoInvent database version 3.9, cut-off, EN15804 model. LCIA Report, Version 1.3
methodology EF v3.1 EN15804.Wernet, G., Bauer, C.,
Steubing, B., Reinhard, J., Moreno-Ruiz, E., and Weidema, B., IBU 2021
2016. The ecoinvent database version 3 (part I): overview and Institut Bauen und Umwelt e.V.: General Instructions for the
methodology. The International Journal of Life Cycle EPD programme of Institut Bauen und Umwelt e.V., Version
Assessment, [online] 21(9), pp.1218–1230. Available at: 2.0, Berlin: Institut Bauen und Umwelt e.V., 2021 http://ibu-
[Accessed 06-01-2023]. epd.com
IBU 2017 SimaPro 2023
PCR Guidance-Text for Building-Related Products and Pré Sustainability,
Services, Part B: Requirements on the EPD for Boards and LCA software SimaPro version 9.5.
panels made of plastic (exterior applications), Version 1.0
7 Environmental Product Declaration - Kima Accessories Aps - Plastic products made of recycled PP or ABS
Publisher
Institut Bauen und Umwelt e.V. +49 (0)30 3087748- 0
Hegelplatz 1 info@ibu-epd.com
10117 Berlin www.ibu-epd.com
Germany
Programme holder
Institut Bauen und Umwelt e.V. +49 (0)30 3087748- 0
Hegelplatz 1 info@ibu-epd.com
10117 Berlin www.ibu-epd.com
Germany
Author of the Life Cycle Assessment
Viegand Maagøe +4533349000
Nørre Farigmagsgade 37 info@viegandmaagoe.dk
1364 Copenhagen www.viegandmaagoe.dk/en
Denmark
Owner of the Declaration
Kima Accessories Aps +4575330800
Kastanievej 3 mail@kimaroof.dk
6862 Tistrup www.kimaroof.dk
Denmark
8 Environmental Product Declaration - Kima Accessories Aps - Plastic products made of recycled PP or ABS
