ENVIRONMENTAL PRODUCT DECLARATION
as per ISO 14025 and EN 15804+A2
Owner of the Declaration ASSA ABLOY Opening Solutions Sweden AB
Programme holder Institut Bauen und Umwelt e.V. (IBU)
Publisher Institut Bauen und Umwelt e.V. (IBU)
Declaration number EPD-ASA-20210013-ICB-EN
Issue date 14.04.2021
Valid to 13.04.2026
ASSA ABLOY PULSE
ASSA ABLOY Opening Solutions
www.ibu-epd.com | https://epd-online.com
Umwelt Produktdeklaration Name des Herstellers – Name des Produkts
1. General Information
ASSA ABLOY Opening Solutions ASSA ABLOY PULSE
Programme holder Owner of the declaration
IBU – Institut Bauen und Umwelt e.V. ASSA ABLOY Opening Solutions Sweden AB
Panoramastr. 1 Kungsgatan 71
10178 Berlin 632 21 Eskilstuna
Germany Sweden
Declaration number Declared product / declared unit
EPD-ASA-20210013-ICB-EN The declaration represents 1 piece of
electromechanical lock cylinder
This declaration is based on the product Scope:
category rules: This study covers the ASSA ABLOY PULSE
Building Hardware products, 02.2016 electromechanical lock cylinder used on the European
(PCR checked and approved by the SVR) market. The key, strike, screws or handle are not
included in the scope.
Issue date
14.04.2021 The calculations and results in the EPD are made for
the round variant of the lock cylinder. The product is
also produced and sold in an oval variant, for which the
Valid to
results in this EPD are representative as a
13.04.2026
conservative estimate. The two variants have the same
composition except for the design and weight of the
cylinder housing. The total weight is 249 grams for the
round version and 130 grams for the oval version. The
results can thus be seen as a conservative estimate
also for the oval version.
The owner of the declaration shall be liable for the
underlying information and evidence; the IBU shall not
be liable with respect to manufacturer information, life
cycle assessment data and evidences.
The EPD was created according to the specifications
of EN 15804+A2. In the following, the standard will be
simplified as EN 15804.
Verification
The standard EN 15804 serves as the core PCR
Independent verification of the declaration and data
according to ISO 14025:2010
Dipl. Ing. Hans Peters internally x externally
(chairman of Institut Bauen und Umwelt e.V.)
Dr. Alexander Röder Dr.-Ing. Wolfram Trinius
(Managing Director Institut Bauen und Umwelt e.V.)) (Independent verifier)
2. Product
2.1 Information about the enterprise With patented features combined with precision
ASSA ABLOY Opening Solutions Sweden AB engineering and cross-function compatibility, the
PULSE cylinder offers:
2.2 Product description/Product definition · High security.
Product name: ASSA ABLOY PULSE · Resistant to picking and manipulation.
· Resistant to bumping.
Product characteristic: · Case-hardened drill-resistant inserts.
Digital locking cylinder with energy harvesting that is · Patented.
completely powered by the insertion of the digital key. Round cylinder with extended security against attack
Key management and accessibility features enable
replacing and adding keys remotely.
For the placing on the market of the products in
the European Union/European Free Trade Association
(EU/EFTA) (with the exception of Switzerland) the
2 Environmental Product Declaration ASSA ABLOY Opening Solutions Sweden AB – ASSA ABLOY PULSE
following harmonization legislation of the European 2.6 Base materials/Ancillary materials
Union applies:
Lock composition
The following directives apply: The average composition for ASSA ABLOY PULSE is
Directive 2014/53/EU of the European Parliament and as following (Round version):
of the Council of 16 April 2014 on the harmonization of Name Value Unit
the laws of the Member States relating to the making Steel 92.73 %
available on the market of radio equipment and Stainless steel 6.69 %
repealing Directive 1999/5/EC Text with European Copper 0.21 %
Economic Area (EEA) relevance - RED Directive Plastics 0.15 %
2014/53/EU Other 0.22 %
Total 100 %
Directive 2011/65/EU of the European Parliament and
of the Council of 8 June 2011 on the restriction of the
use of certain hazardous substances in electrical and 2.7 Manufacture
electronic equipment - RoHS2 2011/65/EU The primary manufacturing processes are made by
Tier 1 suppliers and the final manufacturing processes
and occur in factory Joensuu, Finland.
Commission delegated directive (EU) 2015/863 of 31 The components come from processes like machined
March 2015 amending Annexe II to Directive metal and hardened steel. Final assembly takes place
2011/65/EU of the European Parliament and of the in Finland.
Council as regards the list of restricted substances -
RoHS3 2015/863/EU The factory of Joensuu has a certification of Quality
Management system in accordance with ISO
DoC (document of conformity) reference number 9001:2015.
D0001128671
2.8 Environment and health during
For the application and use of the products the manufacturing
respective national provisions apply ASSA ABLOY Opening Solutions is committed to
producing and distributing door opening solutions with
2.3 Application minimal environmental impact, where health & safety is
ASSA ABLOY PULSE cylinders are suitable for a wide the primary focus for all employees and associates.
range of applications – all from private to commercial
and public sectors, for all types of doors: · Environmental operations, Greenhouse Gas (GHG),
energy, water, waste, Volatile Organic Compound
- Fits in all modern Scandinavian lockcases including (VOC), surface treatment and Health and Safety (H&S)
Evolution- Modul- and 51-series. are being routinely monitored. Inspections, audits, and
- For internal and external use reviews are conducted periodically to ensure that
applicable standards are met, and environmental
2.4 Technical Data management program effectiveness is evaluated.
· Code of Conduct covers human rights, labour
The table presents the technical properties of ASSA practices and decent work. Management of ASSA
ABLOY PULSE cylinders: ABLOY Opening Solutions is aware of their
environmental roles and responsibilities, providing
appropriate training, supporting accountability and
Technical data recognizing outstanding performance.
Name Value Unit
Dimensions (W*H*D or W*H*L) 20 x 35 x mm The factory in Finland has certification of
40 Environmental Management to ISO 14001:2015 and
Weight 0.249 kg Occupational Health and Safety Assessment Series
(round)* (OHSAS) 18001:200:
Supply voltage NA VAC/DC · ISO 9001:2015, FINAS accredited Certificate No.
Power consumption (Stand-by) 54491-2009-AQ-FIN-FINAS
0 mA
· ISO 14001:2015, FINAS accredited Certificate No.
Power consumption (Idle) 0 mA 54494-2009-AE-FIN-FINAS
Power consumption (Peak) 0 mA · OHSAS 18001:2007 FINAS accredited Certificate
Temperature (Operating) -35 to +85 °C No. 54495-2009-AHSO-FIN-FINAS
Temperature (Storage) 0 to +50 °C
*The weight of the oval version of the product is 0.132
kg 2.9 Product processing/Installation
ASSA ABLOY PULSE cylinders are distributed through
and installed by trained installation technicians, such
as locksmiths, carpenters etc. adhering to
2.5 Delivery status local/national standards and requirements. It can also
ASSA ABLOY PULSE cylinders are delivered as be installed by the end user.
separate in a box size – 75 mm x 48 mm x 35 mm
3 Environmental Product Declaration ASSA ABLOY Opening Solutions Sweden AB – ASSA ABLOY PULSE
2.10 Packaging Mechanical destruction
No danger to the environment can be anticipated
ASSA ABLOY PULSE cylinders are packed in a during mechanical destruction
cardboard box with corrugated carton inlays. The
packaging is fully recyclable. Separate package with 2.15 Re-use phase
dimensions: 75 mm x 48 mm x 35 mm The product is possible to re-use during the reference
service life and be moved from one door to another.
2.11 Condition of use 2.16 Disposal
To maintain low friction, bi-annual maintenance <1g of The locks can be mechanically dissembled to separate
oil according to the manufacturer's standard, should be the different materials. The majority, of components is
added inside the cylinder through the profile. steel, stainless steel and copper which can be
Electromechanical cylinders can be replaced or recycled. The plastic components can be used for
upgraded. energy recovery in an incineration plant.
2.12 Environment and health during use 2.17 Further information
There is no harmful emissive potential. No damage to Sweden:
health or impairment is expected under normal use ASSA ABLOY Opening Solutions Sweden AB
corresponding to the intended installation and use of Kungsgatan 71
the product. 63105 Eskilstuna
Sweden +46(0)771640640
2.13 Reference service life Mail: helpdesk.se.openingsolutions@assaabloy.com
Approved for 100.000 cycles under normal working Website: www.assaabloyopeningsolutions.se
conditions.
Norway:
ASSA ABLOY Opening Solutions Norway A/S
2.14 Extraordinary effects Anolitveien 1-3, 1400 Ski
Postboks 424, 1402 Ski
Fire Norge +47 69 24 52 00
Suitable for use in fire and smoke doors. Cylinders Mail helpdesk.no.openingsolutions@assaabloy.com
have been tested and will be classed as Grade B: Website: www.assaabloyopeningsolutions.no
Suitable for use on fire and smoke door assemblies in
accordance with EN 15684. Denmark:
ASSA ABLOY Opening Solutions Denmark A/S
Water Borupvang 5D
Contain no substances that have any impact on water 2750 Ballerup
in case of flood. Electric operation of the device will be Danmark +45 44 54 44 54
influenced negatively. Mail info.dk.openingsolutions@assaabloy.com
Website: www.assaabloyopeningsolutions.dk
3. LCA: Calculation rules
3.1 Declared Unit · C4 – Disposal
The declared unit used in the study is one piece of
electromechanical lock cylinder Beyond system boundary:
· D – Reuse-, recovery- and recycling potential
Declared unit
Name Value Unit Module D includes reuse, recovery and/or recycling
Declared unit piece of piece/prod potential, expressed as net impact and benefits, due to
1
electromechanical lock cylinder uct material recycling.
Mass of declared Product 0.249 kg
3.3 Estimates and assumptions
In the End-of-Life cycle phase, for all the material
3.2 System boundary which can be recycled, a recycling scenario with a 99%
Type of EPD: Cradle to gate - with options collection rate was assumed.
The following life cycle stages were considered:
3.4 Cut-off criteria
Product stage: In the assessment, all available data from the
· A1 – Raw material supply production process are considered.
· A2 – Transport The cut-off criteria in the study follows the rules in EN
· A3 – Manufacturing 15804+A2, Section 6.3.6:
Use stage: · 1% of renewable and non-renewable primary
· B6 – Operational energy use energy usage and 1% of the total mass input of that
unit process
End-of-life stage: · Total neglected input flows per module (e.g. A1-
· C1 – De-construction, demolition A3) shall be a maximum of 5% of energy usage and
· C2 – Transport to waste processing mass
· C3 – Waste processing
4 Environmental Product Declaration ASSA ABLOY Opening Solutions Sweden AB – ASSA ABLOY PULSE
3.5 Background data 3.7 Period under review
Modelling and environmental impact calculations are The period under review is 2019.
performed with the LCA software GaBi (version
9.2.1.68). Generic data and background data are 3.8 Allocation
based on life cycle inventory (LCI) data from GaBi Allocation principles followed EN 15804+A2, Section
Professional database and Ecoinvent 3.6. 6.4. With regards to recycling or other recovery of
waste, impacts are borne by the product until the
3.6 Data quality waste reaches the end-of-waste state. Benefits and
Specific data for the reference year 2019 of the credits of recovery associated with these processes
product, packaging and transport mode and distances are outside the system boundaries.
was collected from ASSA ABLOY and reviewed by
Ramboll LCA practitioners for consistency. The 3.9 Comparability
datasets are complete and conform to the system Basically, a comparison or an evaluation of EPD data
boundaries and the criteria for the exclusion of inputs is only possible if all the data sets to be compared
and outputs. All relevant background datasets are were created according to EN 15804 and the building
taken from the GaBi 2020 Professional database and context, respectively the product-specific
Ecoinvent 3.6. characteristics of performance, are taken into account.
.
4. LCA: Scenarios and additional technical information
Characteristic product properties
Information on biogenic Carbon
Information on describing the biogenic carbon
content at factory gate
Name Value Unit
Biogenic Carbon Content in
- kg C
product
Biogenic Carbon Content in
0.00123 kg C
accompanying packaging
Reference service life not applicable (No impact from
use stage)
End of life (C1-C4)
Name Value Unit
Collected separately
0.246 kg
electromechanical lock
Collected as mixed construction
0.00249 kg
waste electromechanical lock
Recycling of metals 0.245 kg
Landfilling of others 0.001 kg
Reuse, recovery and/or recycling potentials (D),
relevant scenario information
Name Value Unit
Net amount of materials for
0.181 kg
recycling
Whereof recycling steel 96.7 %
Whereof recycling stainless steel 3.0 %
Whereof recycling copper 0.3 %
Whereof recycling brass 0.0 %
No credit has been given in module D for the
corresponding amount of secondary metal entering the
product stage
5 Environmental Product Declaration ASSA ABLOY Opening Solutions Sweden AB – ASSA ABLOY PULSE
5. LCA: Results
Disclaimer:
EP-freshwater: This indicator has been calculated as “kg P eq” as required in the characterization model
(EUTREND model, Struijs et al., 2009b, as implemented in ReCiPe;
http://eplca.jrc.ec.europa.eu/LCDN/developerEF.xhtml)
DESCRIPTION OF THE SYSTEM BOUNDARY (X = INCLUDED IN LCA; ND = MODULE OR INDICATOR NOT
DECLARED; MNR = MODULE NOT RELEVANT)
BENEFITS AND
CONSTRUCTI LOADS
PRODUCT STAGE ON PROCESS USE STAGE END OF LIFE STAGE BEYOND THE
STAGE SYSTEM
BOUNDARIES
6 Environmental Product Declaration ASSA ABLOY Opening Solutions Sweden AB – ASSA ABLOY PULSE
lairetam
waR
ylppus tropsnarT
gnirutcafunaM
eht
morf
tropsnarT
etis
eht
ot
etag
ylbmessA esU
ecnanetniaM
riapeR
tnemecalpeR tnemhsibrufeR
ygrene
lanoitarepO esu
retaw
lanoitarepO esu
noitcurtsnoc-eD
noitilomed tropsnarT
gnissecorp
etsaW
lasopsiD -esueR -yrevoceR -gnilcyceR laitnetop
A1 A2 A3 A4 A5 B1 B2 B3 B4 B5 B6 B7 C1 C2 C3 C4 D
X X X ND ND ND ND MNR MNR MNR X ND X X X X X
RESULTS OF THE LCA - ENVIRONMENTAL IMPACT according to EN 15804+A2: 1 piece
electromechanical lock cylinder
Core Indicator Unit A1-A3 B6 C1 C2 C3 C4 D
GWP-total [kg CO2-Eq.] 9.60E-1 0.00E+0 0.00E+0 9.54E-4 3.84E-2 1.16E-3 -4.34E-1
GWP-fossil [kg CO2-Eq.] 9.70E-1 0.00E+0 0.00E+0 9.48E-4 3.83E-2 2.83E-4 -4.33E-1
GWP-biogenic [kg CO2-Eq.] -1.16E-2 0.00E+0 0.00E+0 -1.59E-6 -3.80E-6 8.72E-4 -2.28E-4
GWP-luluc [kg CO2-Eq.] 8.36E-4 0.00E+0 0.00E+0 7.67E-6 7.99E-5 8.13E-7 -1.34E-4
ODP [kg CFC11-Eq.] 5.76E-9 0.00E+0 0.00E+0 1.74E-19 6.13E-9 -2.55E-19 -4.23E-16
AP [mol H+-Eq.] 6.35E-3 0.00E+0 0.00E+0 1.09E-6 3.10E-4 6.82E-7 -1.60E-3
EP-freshwater [kg PO4-Eq.] 8.04E-5 0.00E+0 0.00E+0 2.89E-9 1.40E-6 1.94E-8 -2.60E-7
EP-marine [kg N-Eq.] 8.71E-4 0.00E+0 0.00E+0 3.36E-7 1.35E-4 3.28E-7 -2.84E-4
EP-terrestrial [mol N-Eq.] 9.49E-3 0.00E+0 0.00E+0 3.99E-6 1.48E-3 2.17E-6 -3.08E-3
POCP [kg NMVOC-Eq.] 2.93E-3 0.00E+0 0.00E+0 9.07E-7 4.04E-4 8.60E-7 -9.23E-4
ADPE [kg Sb-Eq.] 2.66E-5 0.00E+0 0.00E+0 7.66E-11 4.67E-8 9.90E-12 -2.39E-6
ADPF [MJ] 1.12E+1 0.00E+0 0.00E+0 1.26E-2 5.23E-1 3.07E-3 -4.55E+0
[m³ world-Eq
WDP 7.21E-1 0.00E+0 0.00E+0 9.24E-6 1.17E-3 -3.73E-6 -5.19E-1
deprived]
GWP = Global warming potential; ODP = Depletion potential of the stratospheric ozone layer; AP = Acidification potential of land and water; EP =
Caption Eutrophication potential; POCP = Formation potential of tropospheric ozone photochemical oxidants; ADPE = Abiotic depletion potential for non-
fossil resources; ADPF = Abiotic depletion potential for fossil resources; WDP = Water (user) deprivation potential
RESULTS OF THE LCA - INDICATORS TO DESCRIBE RESOURCE USE according to EN 15804+A2: 1 piece
electromechanical lock cylinder
Indicator Unit A1-A3 B6 C1 C2 C3 C4 D
PERE [MJ] 5.81E+0 0.00E+0 0.00E+0 7.31E-4 1.04E-2 7.30E-6 -1.97E-1
PERM [MJ] 4.56E-1 0.00E+0 0.00E+0 0.00E+0 0.00E+0 0.00E+0 0.00E+0
PERT [MJ] 6.27E+0 0.00E+0 0.00E+0 7.31E-4 1.04E-2 7.30E-6 -1.97E-1
PENRE [MJ] 1.12E+1 0.00E+0 0.00E+0 1.27E-2 5.24E-1 3.07E-3 -4.55E+0
PENRM [MJ] 5.01E-2 0.00E+0 0.00E+0 0.00E+0 0.00E+0 0.00E+0 0.00E+0
PENRT [MJ] 1.12E+1 0.00E+0 0.00E+0 1.27E-2 5.24E-1 3.07E-3 -4.55E+0
SM [kg] 6.57E-2 0.00E+0 0.00E+0 0.00E+0 0.00E+0 0.00E+0 0.00E+0
RSF [MJ] 0.00E+0 0.00E+0 0.00E+0 0.00E+0 0.00E+0 0.00E+0 0.00E+0
NRSF [MJ] 0.00E+0 0.00E+0 0.00E+0 0.00E+0 0.00E+0 0.00E+0 0.00E+0
FW [m³] 2.62E-2 0.00E+0 0.00E+0 8.52E-7 3.37E-5 -7.04E-8 -1.22E-2
PERE = Use of renewable primary energy excluding renewable primary energy resources used as raw materials; PERM = Use of
renewable primary energy resources used as raw materials; PERT = Total use of renewable primary energy resources; PENRE = Use of
non-renewable primary energy excluding non-renewable primary energy resources used as raw materials; PENRM = Use of non-
Caption
renewable primary energy resources used as raw materials; PENRT = Total use of non-renewable primary energy resources; SM = Use
of secondary material; RSF = Use of renewable secondary fuels; NRSF = Use of non-renewable secondary fuels; FW = Use of net fresh
water
RESULTS OF THE LCA – WASTE CATEGORIES AND OUTPUT FLOWS according to EN 15804+A2:
1 piece electromechanical lock cylinder
Indicator Unit A1-A3 B6 C1 C2 C3 C4 D
HWD [kg] 1.52E-2 0.00E+0 0.00E+0 5.87E-10 5.81E-9 6.36E-11 -3.29E-7
NHWD [kg] 6.04E-2 0.00E+0 0.00E+0 2.49E-3 9.31E-4 3.23E-3 -3.89E-2
RWD [kg] 4.75E-5 0.00E+0 0.00E+0 2.34E-8 2.32E-7 -4.80E-8 -4.08E-6
CRU [kg] 0.00E+0 0.00E+0 0.00E+0 0.00E+0 0.00E+0 0.00E+0 0.00E+0
MFR [kg] 0.00E+0 0.00E+0 0.00E+0 0.00E+0 2.45E-1 0.00E+0 0.00E+0
MER [kg] 0.00E+0 0.00E+0 0.00E+0 0.00E+0 0.00E+0 0.00E+0 0.00E+0
EEE [MJ] 0.00E+0 0.00E+0 0.00E+0 0.00E+0 0.00E+0 0.00E+0 0.00E+0
EET [MJ] 0.00E+0 0.00E+0 0.00E+0 0.00E+0 0.00E+0 0.00E+0 0.00E+0
HWD = Hazardous waste disposed; NHWD = Non-hazardous waste disposed; RWD = Radioactive waste disposed; CRU = Components
Caption for re-use; MFR = Materials for recycling; MER = Materials for energy recovery; EEE = Exported electrical energy; EEE = Exported
thermal energy
RESULTS OF THE LCA – additional impact categories according to EN 15804+A2-optional:
1 piece electromechanical lock cylinder
Indicator Unit A1-A3 B6 C1 C2 C3 C4 D
[Disease
PM 6.02E-8 0.00E+0 0.00E+0 7.26E-12 7.92E-9 6.92E-12 -2.20E-8
Incidence]
[kBq U235-
IR 1.58E-2 0.00E+0 0.00E+0 3.45E-6 1.90E-3 -8.57E-6 -1.82E-3
Eq.]
ETP-fw [CTUe] 9.16E+0 0.00E+0 0.00E+0 9.46E-3 3.43E-1 2.21E-3 9.13E-1
HTP-c [CTUh] 2.49E-8 0.00E+0 0.00E+0 1.95E-13 1.04E-11 1.09E-13 -7.11E-9
HTP-nc [CTUh] 3.65E-7 0.00E+0 0.00E+0 9.97E-12 3.10E-10 1.04E-11 -4.88E-9
SQP [-] 8.22E+0 0.00E+0 0.00E+0 4.44E-3 9.79E-2 4.20E-4 -2.73E-1
PM = Potential incidence of disease due to PM emissions; IR = Potential Human exposure efficiency relative to U235; ETP-fw = Potential
Caption comparative Toxic Unit for ecosystems; HTP-c = Potential comparative Toxic Unit for humans (cancerogenic); HTP-nc = Potential
comparative Toxic Unit for humans (not cancerogenic); SQP = Potential soil quality index
Disclaimer 1 – for the indicator IRP
This impact category deals mainly with the eventual impact of low dose ionizing
radiation on human health of the nuclear fuel cycle. It does not consider effects due to possible
nuclear accidents, occupational exposure nor due to radioactive waste disposal in underground
facilities. Potential ionizing radiation from the soil, from radon and from some construction materials is also not
measured by this indicator.
Disclaimer 2 – for the indicators ADPE, ADPF, WDP, ETP-fw, HTP-c, HTP-nc, SQP
The results of this environmental impact indicator shall be used with care as the
uncertainties on these results are high or as there is limited experienced with the indicator.
6. LCA: Interpretation
This chapter contains an interpretation of the Life Most of the environmental burden in the majority of the
Cycle Impact Assessment categories. Stated LCIA categories stem from the product stage A1-A3
percentages in the whole interpretation are related to and that a significant net benefit is present from
the overall life cycle. module D. The cylinder housing, which is made of
steel, constitutes 92% of the product by mass and
most of the impact comes from this component of the
product.
The presented results are the impact for ASSA ABLOY
PULSE (round version), which is the product with the
highest environmental impact. If the results would have
been calculated for the oval version, the impacts
related to the production of and waste management of
the cylinder housing materials would have been
lowered since it has less steel in the cylinder housing
and therefore weighs less per declared unit.
The period under review is 2019.
7. Requisite evidence
Not applicable in the EPD.
8. References
DIN EN ISO 9001 DIN EN 15684
ISO 9001:2015, Quality management systems - EN 15684:2012, Building hardware - Mechatronic
Requirements. cylinders - Requirements and test methods.
DIN EN ISO 14001 DIN EN 15804
ISO 14001:2015, Environmental management systems EN 15804:2019+A2, Sustainability of construction
- Requirements with guidance for use. works — Environmental Product Declarations — Core
rules for the product category of construction products.
DIN EN ISO 14025
ISO 14025:2011, Environmental labels and OHSAS 18001
declarations — Type III environmental declarations — OHSAS 18001:2007, Occupational Health and Safety
Principles and procedures. Assessment Series.
Ecoinvent database
ecoinvent center: Ecoinvent 3.6 database.
7 Environmental Product Declaration ASSA ABLOY Opening Solutions Sweden AB – ASSA ABLOY PULSE
Finnish Accreditation Service certificate PCR Part B
ISO 9001:2015, FINAS accredited Certificate No. Institut Bauen und Umwelt e.V.: PCR Part B for
54491-2009-AQ-FIN-FINAS. Building hardware products, version 1.2.
Finnish Accreditation Service certificate Project report
ISO 14001:2015, FINAS accredited Certificate No. Silfverstrand, Niclas; Jelse, Kristian; Palm, David.
54494-2009-AE-FIN-FINAS. Project report: EPD of ASSA ABLOY PULSE. Ramboll
Sweden on behalf of ASSA Abloy EMEA.
Finnish Accreditation Service certificate
OHSAS 18001:2007 FINAS accredited Certificate No. RED directive
54495-2009-AHSO-FIN-FINAS. Directive 2014/53/EU of the European Parliament and
of the Council of 16 April 2014 on the harmonisation of
GaBi software and databases the laws of the Member States relating to the making
Sphera: GaBi 2020 Professional Database, available on the market of radio equipment and
http://www.gabi- repealing Directive 1999/5/EC.
software.com/international/databases/gabi-
databases/professional/, ts 9.2.1.68 incl. databases RoHS2 directive
2020 Edition. Directive 2011/65/EU of the European Parliament and
of the Council of 8 June 2011 on the restriction of the
General instructions use of certain hazardous substances in electrical and
Institut Bauen und Umwelt e.V.: General instructions electronic equipment.
for the EPD programme of Institut Bauen und Umwelt
e.V. (General Instructions for the IBU EPD RoHS3 directive
programme). Version 2.0. Commission delegated directive (EU) 2015/863 of 31
March 2015 amending Annexe II to Directive
PCR Part A 2011/65/EU of the European Parliament and of the
Institut Bauen und Umwelt e.V.: Product Category Council as regards the list of restricted substances.
Rules for Building-Related Products and Services of
Institut Bauen und Umwelt (IBU), Part A: Calculation
Rules for the Life Cycle Assessment and
Requirements on the Project Report according to EN
15804+A2:2019. July 2020.
8 Environmental Product Declaration ASSA ABLOY Opening Solutions Sweden AB – ASSA ABLOY PULSE
Publisher
Institut Bauen und Umwelt e.V. Tel +49 (0)30 3087748- 0
Panoramastr. 1 Fax +49 (0)30 3087748- 29
10178 Berlin Mail info@ibu-epd.com
Germany Web www.ibu-epd.com
Programme holder
Institut Bauen und Umwelt e.V. Tel +49 (0)30 - 3087748- 0
Panoramastr 1 Fax +49 (0)30 – 3087748 - 29
10178 Berlin Mail info@ibu-epd.com
Germany Web www.ibu-epd.com
Author of the Life Cycle
Assessment Tel +46 (0)10 615 60 00
Ramboll Sweden Fax +46 (0)10 615 20 00
Vädursgatan 6 Mail infosverige@ramboll.se
40227 Gothenburg Web www.ramboll.com
Sweden
Owner of the Declaration
ASSA ABLOY Opening Solutions Tel +46(0)771640640
Sweden AB Fax -
Kungsgatan 71 Mail
63105 Eskilstuna helpdesk.se.openingsolutions@a
Sweden ssaabloy.com
Web assaabloyopeningsolutions.se
