Environmental Product Declaration (EPD)
According to ISO 14025 and EN 15804
ACETube®
Registration number: EPD-Kiwa-EE-158059-EN
Issue date: 22-12-2023
Valid until: 22-12-2028
Declaration owner: Gold-Joint Industry Co., Ltd.
Publisher: Kiwa-Ecobility Experts
Program operator: Kiwa-Ecobility Experts
Status: verified
ACETube® | ReTHiNK-58059 1 / 25
Environmental Product Declaration
1 General information
E-mail: marketing@geoace.com
Website: www.geoace.com
1.1 PRODUCT
Production location: Gold-Joint Industry Co., Ltd.
ACETube®
Address production location: No.33, Jing 3 Rd. Wuqi Dist., 43541 Taichung City
1.2 REGISTRATION NUMBER
1.6 VERIFICATION OF THE DECLARATION
EPD-Kiwa-EE-158059-EN
The independent verification is in accordance with the ISO 14025:2011. The LCA is in—
compliance with ISO 14040:2006 and ISO 14044:2006. The EN 15804:2012+A2:2019 serves as—
1.3 VALIDITY
the core PCR.
Issue date: 22-12-2023
Internal ✓ External
Valid until: 22-12-2028
1.4 PROGRAM OPERATOR
Kiwa-Ecobility Experts
Voltastraße 5
13355 Berlin
DE
Elisabeth Amat Guasch, Greenize
1.7 STATEMENTS
Prof. Dr. Frank Heimbecher
The owner of this EPD shall be liable for the underlying information and evidence. The
(Chairman of the independent expert
programme operator Kiwa-Ecobility Experts shall not be liable with respect to
committee - Kiwa-Ecobility Experts)
manufacturer data, life cycle assessment data and evidence.
Frank Huppertz 1.8 PRODUCT CATEGORY RULES
(Head of Kiwa-Ecobility Experts)
Kiwa-Ecobility Experts (Kiwa-EE) – General Product Category Rules (2022-02-14)
Kiwa-Ecobility Experts (Kiwa-EE) – Specific Product Category Rules: Geosynthetic products
1.5 OWNER OF THE DECLARATION
(2023-07-21)
Manufacturer: Gold-Joint Industry Co., Ltd.
Address: No.33, Jing 3 Rd. Wuqi Dist., 43541 Taichung City, Taiwan (R.O.C.)
ACETube® | ReTHiNK-58059 2 / 25
Environmental Product Declaration
1 General information
1.9 COMPARABILITY 1.10 CALCULATION BASIS
In principle, a comparison or assessment of the environmental impacts of different LCA method R<THiNK: Ecobility Experts | EN15804+A2
products is only possible if they have been prepared in accordance with EN 15804. For the
evaluation of the comparability, the following aspects have to be considered in particular: LCA software*: Simapro 9.1
PCR used, functional or declared unit, geographical reference, the definition of the system Characterization method: EN 15804 +A2 Method v1.0
boundary, declared modules, data selection (primary or secondary data, background
database, data quality), scenarios used for use and disposal phases, and the life cycle LCA database profiles: EcoInvent version 3.6
inventory (data collection, calculation methods, allocations, validity period). PCRs and Version database: v3.15 (2023-07-12)
general program instructions of different EPDs programs may differ. Comparability needs
to be evaluated. For further guidance, see EN 15804+A2 (5.3 Comparability of EPD for *Used for calculating the characterized results of the Environmental profiles within
construction products) and ISO 14025 (6.7.2 Requirements for comparability). R<THiNK.
1.11 LCA BACKGROUND REPORT
This EPD is generated on the basis of the LCA background report 'ACETube®' with the
calculation identifier ReTHiNK-58059.
ACETube® | ReTHiNK-58059 3 / 25
Environmental Product Declaration
2 Product
2.1 PRODUCT DESCRIPTION
ACETube® geotextile tubes are tubular-shaped containers fabricated by multiple pieces of
engineered woven fabrics with excellent filtration characteristics. They can be employed as
hydraulic structures for coastal protection and are versatile in various sludge dewatering
applications. Through rigorous in-house and third-party laboratory testing, ACETube® has
demonstrated exceptional durability, including resistance to oxidation, UV, abrasion,
chemicals, and biodegradation. Its superior filtration properties effectively enhance
construction efficiency, leading to significant time and cost savings.
The following products are covered in this EPD: GT50-II PP, GT70-I PP / GT70-I TA, GT70-II
PP, GT100-II PP, GT105-II PP, GT120-II PP, GT175-II PP, GT200-II PP / GT200-II TA, GT250-II PP.
2.2 APPLICATION (INTENDED USE OF THE PRODUCT)
ACETube® geotextile tubes serve as specialized solutions for dewatering and
containment, finding notable applications in environmental and hydraulic engineering.
In the realm of coastal engineering, ACETube® are employed for shoreline protection and
beach nourishment. With the intensification of storm surges and sea-level rise due to
ACETube® | ReTHiNK-58059 4 / 25
Environmental Product Declaration
2 Product
climate change, the tubes' effectiveness in bolstering coastal resilience remains an external partners. Once the warp yarn is prepared or directly placed onto the creel, the
ongoing subject of research. Additionally, ACETube® are utilized in sediment containment weaving process can commence.
efforts. These tubes find use in hydraulic constructions like breakwaters and groins, serving
to protect against tides, currents, waves, and storm surges, while also intended to slow Upon completion of weaving, the fabric is rolled onto beams and sent to our in-house
longshore drift and discourage the mobilization of beach material. processing department for sewing. Given that ACETube® is a customized product, the
processing is conducted according to the specifications, formats, sizes, and accessories
Moreover, these geotextile tubes are deployed for flood control mechanisms. Given the outlined in customer orders. Before sewing operations begin, the fabric is inspected for
increasing frequency of flooding events, they show potential value in creating temporary any weaving defects and then cut according to order requirements. Necessary
barriers or embankments for water containment or diversion. components (e.g., filling ports, handler loops) are then sewn and affixed onto the product.
After assembly, quality control personnel measure the final product's dimensions and
In the environmental sector, ACETube® geotextile tubes are versatile, finding applications count the number of accessories, referencing the production checklist. The sewing areas
in various sludge dewatering scenarios. These include municipal and industrial wastewater are carefully inspected before the product is folded and packaged.
treatment, mining tailings, agricultural animal waste containment, and environmental
dredging, among others.
2.3 REFERENCE SERVICE LIFE
RSL PRODUCT
According to the application standard (EN 13249–13257, EN 13265 and EN 15381), the typical
RSL of ACETube® is about 50 years.
USED RSL (YR) IN THIS LCA CALCULATION:
50
2.4 TECHNICAL DATA
2.7 CONSTRUCTION DESCRIPTION
See above (2.1).
Whether it's a dewatering tube or coastal protection tube, the construction can be divided
into the following parts:
2.5 SUBSTANCES OF VERY HIGH CONCERN
-Layout and positioning
The product contains less than 0.1% of substances included in the “Candidate list of
substances of very high concern for authorisation” (SVHC). -Filling process
-Closure
2.6 DESCRIPTION PRODUCTION PROCESS
ACETube® is crafted from ACETex® PP geotextile, beginning with the tube's formation
through the process of cutting and sewing. This tubular bag is then equipped with
accessory parts (e.g., filling ports, handler loops) as aids for the construction process.
The base material for ACETex® PP woven geotextile is PP yarn. The majority of this yarn is
produced in-house, while some are sourced externally. Prior to weaving, certain PP yarns
are twisted into processed yarns, with operations conducted both internally and by
ACETube® | ReTHiNK-58059 5 / 25
Environmental Product Declaration
2 Product
ACETube® | ReTHiNK-58059 6 / 25
Environmental Product Declaration
3 Calculation rules
3.1 DECLARED UNIT Module B2 = Maintenance Module C4 = Disposal
Module D = Benefits and loads beyond the
One square meter ACETube® Module B3 = Repair
product system boundaries
One square meter of ACETube®. The following products are covered in this EPD: GT50-II
Module B4 = Replacement
PP, GT70-I PP / GT70-I TA, GT70-II PP, GT100-II PP, GT105-II PP, GT120-II PP, GT175-II PP,
GT200-II PP / GT200-II TA, GT250-II PP.
reference_unit: square meter (m2) 3.4 REPRESENTATIVENESS
The input data are representative for ACETube®, a product of Gold-Joint Industry. The data
3.2 CONVERSION FACTORS
are representative for Asia.
Description Value Unit
3.5 CUT-OFF CRITERIA
reference_unit 1 m2
weight_per_reference_unit 1.309 kg Product Stage (A1-A3)
Conversion factor to 1 kg 0.763930 m2
The following inputs have been placed under cut-off criteria (<2% of the total mass):
3.3 SCOPE OF DECLARATION AND SYSTEM BOUNDARIES -Raw materials : PET, HDPE, PP webbing
This is a Cradle to gate with options, modules C1-C4 and module D LCA. The life cycle Construction process stage (A4-A5)
stages included are as shown below:
(X = module included, ND = module not declared) This stage consists the transport of the product from production plant to the construction
site.
A1 A2 A3 A4 A5 B1 B2 B3 B4 B5 B6 B7 C1 C2 C3 C4 D
X X X X X ND ND ND ND ND ND ND X X X X X It also includes the loss of material during construction. The additional needed production,
transport and end-of-life of the lost material during construction is included.
The end-of-life of packaging material up to the end-of-waste state or disposal of final
The modules of the EN15804 contain the following:
residues is also included.
Module A1 = Raw material supply Module B5 = Refurbishment
End of life stage (C1-C4)
Module A2 = Transport Module B6 = Operational energy use
Module A3 = Manufacturing Module B7 = Operational water use
When the end of the life stage of the building is reached, the de-construction/demolition
Module A4 = Transport Module C1 = De-construction / Demolition
begins. This EPD includes de-construction/demolition (C1), the necessary transport (C2)
Module A5 = Construction - from the demolition site to the sorting location and distance to final disposal. The end of
Module C2 = Transport life stage includes the final disposal to landfill (C4), incineration (C3) and needed recycling
Installation process
processes up to the end-of-waste point (C3). Loads and benefits of recycling, re-use and
Module B1 = Use Module C3 = Waste Processing exported energy are part of module D.
ACETube® | ReTHiNK-58059 7 / 25
Environmental Product Declaration
3 Calculation rules
The prescribed waste scenarios from the NMD Determination method v1.0 have been used A scaling method was used to calculate the LCA results for the different ACETube®
for the various materials in the product. products. The scaling was done on the basis of mass per square meter. As a result of
scaling there are results for both the fixed and the scalable part of the scaling function.
The fixed part means that this number is the same for each product in the product group
Benefits and Loads beyond the system boundary (Module D) and the scalable part is the part that depends on the mass per unit area of the product. In
order to calculate the correct number of each environmental impact category for each of
the products in the product group, the following calculation should be done:
This stage contains the potential loads and benefits of recycling and re-use of raw
materials/products. The loads contain the needed recycling processes from end-of-waste- [number fixed part]+([specific mass]*[number scalable part])
point up to the point-of-equivalence of the substituted primary raw material and a load for
secondary material that will be lost at the end-of-life stage. The inputs of PET raw yarn and PET webbing did not have a linear dependence on the
specific mass, so the higher amount of product available was always considered for scaling
The loads and benefits of recycling and reuse are included in this module. The benefits are to be as conservative as possible.
calculated based on the primary content and the primary equivalent.
The inputs PP raw yarn, PP chips and PE chips also did not have a linear dependence on
In addition, the benefits of energy recovery are granted at this stage. The amount of avoid the specific mass. As they are the main inputs present in the product, the linear
energy is based on the Lower Heating Values of the materials and the efficiencies of the dependence on the specific mass of the sum of these 3 inputs was calculated instead of
incinerators as mentioned in the NMD Determination method v1.0 or EcoInvent 3.6 (2019). considering the inputs separately.
The linear dependence of the energy consumption on the specific mass has been
3.6 ALLOCATION calculated by taking into account the sum of the production energy and the yarn wisting
energy (which is outsourced).
Allocation is based on physical characteristics, on mass. The production data was
calculated according to the annual quantity by mass. The raw materials and energy were For C1 the method and amount of the generic data set 'Polyester weefsel' from chapter
calculated according to this allocation key. 22.46 Grondwapening en grondscheiding of the DuboCalc programme (database version
NMD 1.8 - 5.01.14052018) was used. In this generic data set, 0.0013h work per m² of
geotextile was assumed.
3.7 DATA COLLECTION & REFERENCE TIME PERIOD
All process-specific data was collected for the operating year 2021. 3.9 DATA QUALITY
All process-specific data was collected for the 2021 operating year and is therefore up-to-
3.8 ESTIMATES AND ASSUMPTIONS date. The data is based on the annual average. In order to ensure comparability of the
results, only consistent background data of the Ecoinvent database V3.6 was used in the
Almost all the datasets selected for the LCA refer to the RoW as the geographical LCA (e.g., records on energy, transportation, and supplies), which refers to reference year
reference, as there were no specific environmental profiles available. 2019. The database is regularly reviewed and thus complies with the requirements of EN
15804 (background data not older than 10 years). All consistent datasets contained in the
Gold-Joint delivers its product to different countries, so the calculation of transport to Ecoinvent database are documented and can be viewed in the online Ecoinvent
construction site (A4) was done by taking the average distance, weighted by the documentation. The primary data were provided by Gold-Joint. The life cycle was modelled
proportion of product shipped to each country. For module A4, a data set for a non- with the R<THiNK EPD App.
specific truck and a transoceanic ship was used.
The following inputs have been placed under cut-off criteria (<2% of the total mass): 3.10 GUARANTEES OF ORIGIN
-Raw materials : PET, HDPE, PP webbing
In this EPD, the local based approach was considered for the LCA, therefore no guaranties
of origin (GO) are needed.
ACETube® | ReTHiNK-58059 8 / 25
Environmental Product Declaration
3 Calculation rules
3.12 SCALING
Parameter Value
Scaling type Linear
Description dimension mass
Dimension 0.000
Scalable dimension 1.000
Unit dimension kg/m²
ACETube® | ReTHiNK-58059 9 / 25
Environmental Product Declaration
4 Scenarios and additional technical information
4.1 TRANSPORT TO CONSTRUCTION SITE (A4)
For the transport from production place to assembly/user, the following scenario is
assumed for module A4 of this EPD.
Value and unit
Vehicle type used for transport Transoceanic ship / Lorry unspecified
Fuel type and consumption of vehicle
Distance 5157 km
Capacity utilisation (including empty returns)
Bulk density of transported products
Volume capacity utilisation factor
4.2 ASSEMBLY (A5)
The following information describes the scenarios for flows entering the system and flows
leaving the system at module A5.
FLOWS ENTERING THE SYSTEM
There are no significant environment impacts as a result of materials or energy used in the
construction stage (A5).
FLOWS LEAVING THE SYSTEM
The following output flows leaving the system at module A5 are assumed.
Description Value Unit
Output materials as result of loss during construction 5 %
Output materials as result of waste processing of materials used for installation/assembly at the building site 0.000 kg
Output materials as result of waste processing of used packaging 0.046 kg
4.3 DE-CONSTRUCTION, DEMOLITION (C1)
The following information describes the scenario for demolition at end of life.
Description Amount Unit
Hydraulic excavator (average) [NMD] 0.001 hr
ACETube® | ReTHiNK-58059 10 / 25
Environmental Product Declaration
4 Scenarios and additional technical information
4.4 TRANSPORT END-OF-LIFE (C2)
The following distances and transport conveyance are assumed for transportation during
end of life for the different types of waste processing.
Waste Scenario Transport conveyance Not removed (stays in Landfill Incineration Recycling Re-use
work) [km] [km] [km] [km] [km]
PE/PP soil reinforcement (geotextile and Lorry (Truck), unspecified (default) | market
0 100 150 50 0
geogrid 54) group for (GLO)
The transport conveyance(s) used in the scenario(s) for transport during end of life has the
following characteristics.
Value and unit
Vehicle type used for transport Lorry (Truck), unspecified (default) | market group for (GLO)
Fuel type and consumption of vehicle not available
Capacity utilisation (including empty returns) 50 % (loaded up and return empty)
Bulk density of transported products inapplicable
Volume capacity utilisation factor 1
4.5 END OF LIFE (C3, C4)
The scenario(s) assumed for end of life of the product are given in the following tables.
First the assumed percentages per type of waste processing are displayed, followed by the
assumed amounts.
Waste Scenario Region Not removed (stays in work) [%] Landfill [%] Incineration [%] Recycling [%] Re-use [%]
PE/PP soil reinforcement (geotextile and geogrid 54) NL 25 0 70 5 0
Waste Scenario Not removed (stays in work) [kg] Landfill [kg] Incineration [kg] Recycling [kg] Re-use [kg]
PE/PP soil reinforcement (geotextile and geogrid 54) 0.344 0.000 0.964 0.069 0.000
Total 0.344 0.000 0.964 0.069 0.000
ACETube® | ReTHiNK-58059 11 / 25
Environmental Product Declaration
4 Scenarios and additional technical information
4.6 BENEFITS AND LOADS BEYOND THE SYSTEM BOUNDARY (D)
The presented Benefits and loads beyond the system boundary in this EPD are based on
the following calculated Net output flows in kilograms and Energy recovery displayed in
MJ Lower Heating Value.
Waste Scenario Net output flow [kg] Energy recovery [MJ]
PE/PP soil reinforcement (geotextile and geogrid 54) 0.065 31.499
Total 0.065 31.499
ACETube® | ReTHiNK-58059 12 / 25
Environmental Product Declaration
5 Results
For the impact assessment, the characterization factors of the LCIA method EN 15804 +A2
Method v1.0 are used. Long-term emissions (>100 years) are not considered in the impact
assessment. The results of the impact assessment are only relative statements that do not
make any statements about end-points of the impact categories, exceedance of threshold
values, safety margins or risks. The following tables show the results of the indicators of the
impact assessment, of the use of resources as well as of waste and other output flows.
ACETube® | ReTHiNK-58059 13 / 25
Environmental Product Declaration
5 Results
5.1 ENVIRONMENTAL IMPACT INDICATORS PER SQUARE METER (FIXED PART)
CORE ENVIRONMENTAL IMPACT INDICATORS EN15804+A2
Abbreviation Unit A1 A2 A3 A4 A5 C1 C2 C3 C4 D
AP mol H+ eqv. -6.70E-4 -1.67E-6 -2.54E-4 -1.06E-4 -5.25E-5 7.12E-4 -5.43E-6 -5.46E-5 -1.49E-6 7.71E-5
GWP-total kg CO2 eqv. -1.65E-1 -6.28E-4 -6.52E-2 -9.07E-3 -8.96E-3 6.81E-2 -9.36E-4 -1.21E-1 -2.39E-3 7.18E-2
GWP-b kg CO2 eqv. -2.51E-4 -3.46E-7 1.58E-4 -5.61E-6 8.57E-3 1.89E-5 -4.32E-7 -1.75E-5 -1.84E-6 5.23E-5
GWP-f kg CO2 eqv. -1.64E-1 -6.28E-4 -6.54E-2 -9.06E-3 -1.75E-2 6.81E-2 -9.35E-4 -1.21E-1 -2.39E-3 7.18E-2
GWP-luluc kg CO2 eqv. -7.63E-5 -2.06E-7 2.07E-5 -3.75E-6 -3.34E-6 5.37E-6 -3.43E-7 -9.84E-6 -8.45E-8 1.82E-6
EP-m kg N eqv. -1.18E-4 -8.44E-7 -3.08E-5 -2.64E-5 -8.86E-6 3.14E-4 -1.91E-6 -1.49E-5 -9.03E-7 2.00E-5
EP-fw kg P eqv. -3.87E-6 -6.77E-9 -1.77E-6 -1.07E-7 -3.01E-7 2.48E-7 -9.44E-9 -3.65E-7 -3.07E-9 1.72E-7
EP-T mol N eqv. -1.31E-3 -9.25E-6 -3.55E-4 -2.94E-4 -9.93E-5 3.45E-3 -2.11E-5 -1.66E-4 -5.48E-6 2.20E-4
kg CFC 11
ODP -3.82E-9 -1.40E-10 -2.88E-9 -1.93E-9 -5.87E-10 1.47E-8 -2.06E-10 -3.70E-9 -5.29E-11 8.61E-9
eqv.
kg NMVOC
POCP -5.31E-4 -2.82E-6 -1.29E-4 -8.05E-5 -3.72E-5 9.49E-4 -6.02E-6 -4.47E-5 -2.10E-6 7.97E-5
eqv.
ADP-f MJ -5.05E+0 -9.64E-3 -9.23E-1 -1.34E-1 -3.10E-1 9.37E-1 -1.41E-2 -9.44E-2 -4.05E-3 1.33E+0
ADP-mm kg Sb-eqv. -1.63E-6 -1.72E-8 -1.43E-7 -1.59E-7 -9.66E-8 1.04E-7 -2.37E-8 -1.55E-7 -1.83E-9 7.63E-8
m3 world
WDP -6.70E-2 -3.65E-5 -8.93E-3 -5.88E-4 -4.11E-3 1.26E-3 -5.05E-5 -6.18E-3 -1.73E-4 1.02E-2
eqv.
AP=Acidification (AP) | GWP-total=Global warming potential (GWP-total) | GWP-b=Global warming potential - Biogenic (GWP-b) | GWP-f=Global warming potential - Fossil (GWP-f) | GWP-
luluc=Global warming potential - Land use and land use change (GWP-luluc) | EP-m=Eutrophication marine (EP-m) | EP-fw=Eutrophication, freshwater (EP-fw) | EP-T=Eutrophication,
terrestrial (EP-T) | ODP=Ozone depletion (ODP) | POCP=Photochemical ozone formation - human health (POCP) | ADP-f=Resource use, fossils (ADP-f) | ADP-mm=Resource use, minerals and
metals (ADP-mm) | WDP=Water use (WDP)
ACETube® | ReTHiNK-58059 14 / 25
Environmental Product Declaration
5 Results
ADDITIONAL ENVIRONMENTAL IMPACT INDICATORS EN15084+A2
Abbreviation Unit A1 A2 A3 A4 A5 C1 C2 C3 C4 D
ETP-fw CTUe -1.96E+0 -8.83E-3 -3.64E-1 -1.10E-1 -1.84E-1 5.65E-1 -1.26E-2 -1.52E+0 -4.30E-3 9.98E-2
disease
PM -5.23E-9 -6.08E-11 -5.17E-10 -6.41E-10 -3.17E-10 1.89E-8 -8.42E-11 -4.42E-10 -2.81E-11 3.46E-10
incidence
HTP-c CTUh -3.96E-11 -2.64E-13 -1.12E-11 -3.62E-12 -3.17E-12 1.97E-11 -4.08E-13 -2.32E-11 -1.13E-13 5.80E-12
HTP-nc CTUh -1.24E-9 -9.83E-12 -4.37E-10 -1.12E-10 -1.06E-10 4.85E-10 -1.38E-11 -4.81E-10 -2.80E-12 9.76E-11
IR kBq U235 eqv. -2.36E-3 -4.03E-5 -2.45E-3 -5.71E-4 -2.78E-4 4.02E-3 -5.91E-5 -3.86E-4 -1.58E-5 5.04E-4
SQP Pt -2.10E-1 -9.05E-3 6.95E-2 -8.53E-2 -1.28E-2 1.20E-1 -1.22E-2 -3.48E-2 -9.56E-3 -2.39E-1
ETP-fw=Ecotoxicity, freshwater (ETP-fw) | PM=Particulate Matter (PM) | HTP-c=Human toxicity, cancer (HTP-c) | HTP-nc=Human toxicity, non-cancer (HTP-nc) | IR=Ionising radiation, human
health (IR) | SQP=Land use (SQP)
CLASSIFICATION OF DISCLAIMERS TO THE DECLARATION OF CORE AND ADDITIONAL ENVIRONMENTAL IMPACT INDICATORS
ILCD classification Indicator Disclaimer
Global warming potential (GWP) None
ILCD type / level 1 Depletion potential of the stratospheric ozone layer (ODP) None
Potential incidence of disease due to PM emissions (PM) None
AAcidification potential, Accumulated Exceedance (AP) None
Eutrophication potential, Fraction of nutrients reaching freshwater end compartment
None
(EP-freshwater)
Eutrophication potential, Fraction of nutrients reaching marine end compartment
ILCD type / level 2 None
(EP-marine)
Eutrophication potential, Accumulated Exceedance (EP-terrestrial) None
Formation potential of tropospheric ozone (POCP) None
Potential Human exposure efficiency relative to U235 (IRP) 1
Abiotic depletion potential for non-fossil resources (ADP-minerals&metals) 2
ILCD type / level 3
Abiotic depletion potential for fossil resources (ADP-fossil) 2
Water (user) deprivation potential, deprivation-weighted water consumption (WDP) 2
Potential Comparative Toxic Unit for ecosystems (ETP-fw) 2
ACETube® | ReTHiNK-58059 15 / 25
Environmental Product Declaration
5 Results
ILCD classification Indicator Disclaimer
Potential Comparative Toxic Unit for humans (HTP-c) 2
Potential Comparative Toxic Unit for humans (HTP-nc) 2
Potential Soil quality index (SQP) 2
Disclaimer 1 – This impact category deals mainly with the eventual impact of low dose ionizing radiation on human health of the nuclear fuel cycle. It does not consider effects due to possible
nuclear accidents, occupational exposure nor due to radioactive waste disposal in underground facilities. Potential ionizing radiation from the soil, from radon and from some construction
materials is also not measured by this indicator.
Disclaimer 2 – The results of this environmental impact indicator shall be used with care as the uncertainties on these results are high or as there is limited experienced with the indicator.
5.2 ENVIRONMENTAL IMPACT INDICATORS PER SQUARE METER (SCALABLE PART)
CORE ENVIRONMENTAL IMPACT INDICATORS EN15804+A2
Abbreviation Unit A1 A2 A3 A4 A5 C1 C2 C3 C4 D
AP mol H+ eqv. 1.43E-2 1.99E-5 1.88E-3 2.54E-3 1.05E-3 0.00E+0 1.16E-4 1.16E-3 3.18E-5 -1.77E-3
GWP-total kg CO2 eqv. 3.45E+0 3.43E-3 5.17E-1 2.16E-1 4.44E-1 0.00E+0 1.99E-2 2.58E+0 5.10E-2 -1.66E+0
GWP-b kg CO2 eqv. 8.00E-3 1.58E-6 -4.70E-4 1.34E-4 4.23E-4 0.00E+0 9.20E-6 3.73E-4 3.92E-5 -1.16E-3
GWP-f kg CO2 eqv. 3.44E+0 3.43E-3 5.18E-1 2.16E-1 4.43E-1 0.00E+0 1.99E-2 2.58E+0 5.09E-2 -1.66E+0
GWP-luluc kg CO2 eqv. 1.87E-3 1.26E-6 1.36E-4 8.95E-5 1.24E-4 0.00E+0 7.30E-6 2.10E-4 1.80E-6 -8.81E-5
EP-m kg N eqv. 2.52E-3 7.00E-6 2.90E-4 6.30E-4 2.06E-4 0.00E+0 4.07E-5 3.18E-4 1.92E-5 -4.62E-4
EP-fw kg P eqv. 8.38E-5 3.46E-8 1.22E-5 2.55E-6 5.64E-6 0.00E+0 2.01E-7 7.77E-6 6.53E-8 -4.13E-6
EP-T mol N eqv. 2.80E-2 7.72E-5 3.24E-3 7.02E-3 2.29E-3 0.00E+0 4.49E-4 3.54E-3 1.17E-4 -5.09E-3
kg CFC 11
ODP 1.17E-7 7.56E-10 1.68E-8 4.60E-8 1.69E-8 0.00E+0 4.40E-9 7.89E-8 1.13E-9 -2.00E-7
eqv.
kg NMVOC
POCP 1.12E-2 2.20E-5 1.31E-3 1.92E-3 8.24E-4 0.00E+0 1.28E-4 9.51E-4 4.47E-5 -1.84E-3
eqv.
AP=Acidification (AP) | GWP-total=Global warming potential (GWP-total) | GWP-b=Global warming potential - Biogenic (GWP-b) | GWP-f=Global warming potential - Fossil (GWP-f) | GWP-
luluc=Global warming potential - Land use and land use change (GWP-luluc) | EP-m=Eutrophication marine (EP-m) | EP-fw=Eutrophication, freshwater (EP-fw) | EP-T=Eutrophication,
terrestrial (EP-T) | ODP=Ozone depletion (ODP) | POCP=Photochemical ozone formation - human health (POCP) | ADP-f=Resource use, fossils (ADP-f) | ADP-mm=Resource use, minerals and
metals (ADP-mm) | WDP=Water use (WDP)
ACETube® | ReTHiNK-58059 16 / 25
Environmental Product Declaration
5 Results
Abbreviation Unit A1 A2 A3 A4 A5 C1 C2 C3 C4 D
ADP-f MJ 1.05E+2 5.17E-2 9.25E+0 3.20E+0 6.13E+0 0.00E+0 3.01E-1 2.01E+0 8.62E-2 -3.05E+1
ADP-mm kg Sb-eqv. 3.54E-5 8.68E-8 3.33E-6 3.78E-6 2.47E-6 0.00E+0 5.05E-7 3.31E-6 3.90E-8 -1.72E-6
m3 world
WDP 1.31E+0 1.85E-4 1.16E-1 1.40E-2 8.41E-2 0.00E+0 1.08E-3 1.32E-1 3.69E-3 -2.28E-1
eqv.
AP=Acidification (AP) | GWP-total=Global warming potential (GWP-total) | GWP-b=Global warming potential - Biogenic (GWP-b) | GWP-f=Global warming potential - Fossil (GWP-f) | GWP-
luluc=Global warming potential - Land use and land use change (GWP-luluc) | EP-m=Eutrophication marine (EP-m) | EP-fw=Eutrophication, freshwater (EP-fw) | EP-T=Eutrophication,
terrestrial (EP-T) | ODP=Ozone depletion (ODP) | POCP=Photochemical ozone formation - human health (POCP) | ADP-f=Resource use, fossils (ADP-f) | ADP-mm=Resource use, minerals and
metals (ADP-mm) | WDP=Water use (WDP)
ADDITIONAL ENVIRONMENTAL IMPACT INDICATORS EN15084+A2
Abbreviation Unit A1 A2 A3 A4 A5 C1 C2 C3 C4 D
ETP-fw CTUe 4.09E+1 4.61E-2 6.85E+0 2.63E+0 5.40E+0 0.00E+0 2.68E-1 3.24E+1 9.17E-2 -2.29E+0
disease
PM 1.17E-7 3.08E-10 1.08E-8 1.53E-8 8.19E-9 0.00E+0 1.79E-9 9.42E-9 5.99E-10 -7.90E-9
incidence
HTP-c CTUh 8.62E-10 1.49E-12 1.28E-10 8.63E-11 9.83E-11 0.00E+0 8.69E-12 4.94E-10 2.40E-12 -1.34E-10
HTP-nc CTUh 2.57E-8 5.04E-11 3.80E-9 2.67E-9 2.54E-9 0.00E+0 2.93E-10 1.03E-8 5.97E-11 -2.25E-9
IR kBq U235 eqv. 6.60E-2 2.16E-4 1.32E-2 1.36E-2 5.53E-3 0.00E+0 1.26E-3 8.23E-3 3.37E-4 -1.16E-2
SQP Pt 4.76E+0 4.48E-2 6.69E-1 2.03E+0 4.77E-1 0.00E+0 2.61E-1 7.40E-1 2.04E-1 -5.34E-1
ETP-fw=Ecotoxicity, freshwater (ETP-fw) | PM=Particulate Matter (PM) | HTP-c=Human toxicity, cancer (HTP-c) | HTP-nc=Human toxicity, non-cancer (HTP-nc) | IR=Ionising radiation, human
health (IR) | SQP=Land use (SQP)
CLASSIFICATION OF DISCLAIMERS TO THE DECLARATION OF CORE AND ADDITIONAL ENVIRONMENTAL IMPACT INDICATORS
ILCD classification Indicator Disclaimer
Global warming potential (GWP) None
ILCD type / level 1 Depletion potential of the stratospheric ozone layer (ODP) None
Potential incidence of disease due to PM emissions (PM) None
AAcidification potential, Accumulated Exceedance (AP) None
ILCD type / level 2
None
ACETube® | ReTHiNK-58059 17 / 25
Environmental Product Declaration
5 Results
ILCD classification Indicator Disclaimer
Eutrophication potential, Fraction of nutrients reaching freshwater end compartment
(EP-freshwater)
Eutrophication potential, Fraction of nutrients reaching marine end compartment
None
(EP-marine)
Eutrophication potential, Accumulated Exceedance (EP-terrestrial) None
Formation potential of tropospheric ozone (POCP) None
Potential Human exposure efficiency relative to U235 (IRP) 1
Abiotic depletion potential for non-fossil resources (ADP-minerals&metals) 2
Abiotic depletion potential for fossil resources (ADP-fossil) 2
Water (user) deprivation potential, deprivation-weighted water consumption (WDP) 2
ILCD type / level 3 Potential Comparative Toxic Unit for ecosystems (ETP-fw) 2
Potential Comparative Toxic Unit for humans (HTP-c) 2
Potential Comparative Toxic Unit for humans (HTP-nc) 2
Potential Soil quality index (SQP) 2
Disclaimer 1 – This impact category deals mainly with the eventual impact of low dose ionizing radiation on human health of the nuclear fuel cycle. It does not consider effects due to possible
nuclear accidents, occupational exposure nor due to radioactive waste disposal in underground facilities. Potential ionizing radiation from the soil, from radon and from some construction
materials is also not measured by this indicator.
Disclaimer 2 – The results of this environmental impact indicator shall be used with care as the uncertainties on these results are high or as there is limited experienced with the indicator.
ACETube® | ReTHiNK-58059 18 / 25
Environmental Product Declaration
5 Results
5.3 ENVIRONMENTAL IMPACT INDICATORS PER SQUARE METER (FIXED PART)
PARAMETERS DESCRIBING RESOURCE USE
Abbreviation Unit A1 A2 A3 A4 A5 C1 C2 C3 C4 D
PERE MJ -7.44E-2 -1.26E-4 -6.64E-3 -2.00E-3 -4.49E-3 5.07E-3 -1.77E-4 -9.55E-3 -7.16E-5 -3.89E-2
PERM MJ 0.00E+0 0.00E+0 0.00E+0 0.00E+0 0.00E+0 0.00E+0 0.00E+0 0.00E+0 0.00E+0 0.00E+0
PERT MJ -7.44E-2 -1.26E-4 -6.64E-3 -2.00E-3 -4.49E-3 5.07E-3 -1.77E-4 -9.55E-3 -7.16E-5 -3.89E-2
PENRE MJ -2.89E+0 -1.02E-2 -9.60E-1 -1.42E-1 -2.05E-1 9.95E-1 -1.50E-2 -1.00E-1 -4.30E-3 1.32E+0
PENRM MJ -2.52E+0 0.00E+0 -1.88E-2 0.00E+0 -1.27E-1 0.00E+0 0.00E+0 0.00E+0 0.00E+0 1.44E-1
PENRT MJ -5.41E+0 -1.02E-2 -9.79E-1 -1.42E-1 -3.32E-1 9.95E-1 -1.50E-2 -1.00E-1 -4.30E-3 1.46E+0
SM Kg 0.00E+0 0.00E+0 0.00E+0 0.00E+0 0.00E+0 0.00E+0 0.00E+0 0.00E+0 0.00E+0 0.00E+0
RSF MJ 0.00E+0 0.00E+0 0.00E+0 0.00E+0 0.00E+0 0.00E+0 0.00E+0 0.00E+0 0.00E+0 0.00E+0
NRSF MJ 0.00E+0 0.00E+0 0.00E+0 0.00E+0 0.00E+0 0.00E+0 0.00E+0 0.00E+0 0.00E+0 0.00E+0
FW M3 -1.67E-3 -1.24E-6 -2.49E-4 -1.93E-5 -1.04E-4 4.83E-5 -1.72E-6 -1.82E-4 -4.22E-6 1.44E-4
PERE=renewable primary energy ex. raw materials | PERM=renewable primary energy used as raw materials | PERT=renewable primary energy total | PENRE=non-renewable primary energy
ex. raw materials | PENRM=non-renewable primary energy used as raw materials | PENRT=non-renewable primary energy total | SM=use of secondary material | RSF=use of renewable
secondary fuels | NRSF=use of non-renewable secondary fuels | FW=use of net fresh water
OTHER ENVIRONMENTAL INFORMATION DESCRIBING WASTE CATEGORIES
Abbreviation Unit A1 A2 A3 A4 A5 C1 C2 C3 C4 D
HWD Kg -5.84E-7 -2.59E-8 -3.14E-7 -2.66E-7 -6.30E-8 2.55E-6 -3.58E-8 -1.80E-7 -6.15E-9 1.40E-6
NHWD Kg -9.00E-3 -6.69E-4 -3.19E-3 -5.82E-3 -1.74E-3 1.11E-3 -8.95E-4 -2.33E-3 -1.62E-2 6.10E-4
RWD Kg -1.99E-6 -6.29E-8 -2.21E-6 -8.78E-7 -2.57E-7 6.51E-6 -9.26E-8 -3.39E-7 -2.40E-8 6.54E-7
HWD=hazardous waste disposed | NHWD=non hazardous waste disposed | RWD=radioactive waste disposed
ACETube® | ReTHiNK-58059 19 / 25
Environmental Product Declaration
5 Results
ENVIRONMENTAL INFORMATION DESCRIBING OUTPUT FLOWS
Abbreviation Unit A1 A2 A3 A4 A5 C1 C2 C3 C4 D
CRU Kg 0.00E+0 0.00E+0 0.00E+0 0.00E+0 0.00E+0 0.00E+0 0.00E+0 0.00E+0 0.00E+0 0.00E+0
MFR Kg 0.00E+0 0.00E+0 -1.55E-4 0.00E+0 3.78E-3 0.00E+0 0.00E+0 -3.22E-3 0.00E+0 0.00E+0
MER Kg 0.00E+0 0.00E+0 0.00E+0 0.00E+0 0.00E+0 0.00E+0 0.00E+0 0.00E+0 0.00E+0 0.00E+0
EET MJ 0.00E+0 0.00E+0 -2.34E-2 0.00E+0 0.00E+0 0.00E+0 0.00E+0 0.00E+0 0.00E+0 -4.84E-1
EEE MJ 0.00E+0 0.00E+0 -1.36E-2 0.00E+0 0.00E+0 0.00E+0 0.00E+0 0.00E+0 0.00E+0 -2.81E-1
CRU=Components for re-use | MFR=Materials for recycling | MER=Materials for energy recovery | EET=Exported Energy Thermic | EEE=Exported Energy Electric
5.4 ENVIRONMENTAL IMPACT INDICATORS PER SQUARE METER (SCALABLE PART)
PARAMETERS DESCRIBING RESOURCE USE
Abbreviation Unit A1 A2 A3 A4 A5 C1 C2 C3 C4 D
PERE MJ 1.69E+0 6.47E-4 2.33E-1 4.77E-2 1.17E-1 0.00E+0 3.76E-3 2.03E-1 1.53E-3 -1.41E-1
PERM MJ 0.00E+0 0.00E+0 0.00E+0 0.00E+0 0.00E+0 0.00E+0 0.00E+0 0.00E+0 0.00E+0 0.00E+0
PERT MJ 1.69E+0 6.47E-4 2.33E-1 4.77E-2 1.17E-1 0.00E+0 3.76E-3 2.03E-1 1.53E-3 -1.41E-1
PENRE MJ 6.31E+1 5.48E-2 6.22E+0 3.39E+0 3.93E+0 0.00E+0 3.19E-1 2.14E+0 9.16E-2 -3.05E+1
PENRM MJ 4.90E+1 0.00E+0 3.63E+0 0.00E+0 2.64E+0 0.00E+0 0.00E+0 0.00E+0 0.00E+0 -3.13E+0
PENRT MJ 1.12E+2 5.48E-2 9.85E+0 3.39E+0 6.57E+0 0.00E+0 3.19E-1 2.14E+0 9.16E-2 -3.36E+1
SM Kg 0.00E+0 0.00E+0 0.00E+0 0.00E+0 0.00E+0 0.00E+0 0.00E+0 0.00E+0 0.00E+0 0.00E+0
RSF MJ 0.00E+0 0.00E+0 0.00E+0 0.00E+0 0.00E+0 0.00E+0 0.00E+0 0.00E+0 0.00E+0 0.00E+0
NRSF MJ 0.00E+0 0.00E+0 0.00E+0 0.00E+0 0.00E+0 0.00E+0 0.00E+0 0.00E+0 0.00E+0 0.00E+0
FW M3 3.27E-2 6.29E-6 3.13E-3 4.60E-4 2.17E-3 0.00E+0 3.66E-5 3.87E-3 8.99E-5 -3.24E-3
PERE=renewable primary energy ex. raw materials | PERM=renewable primary energy used as raw materials | PERT=renewable primary energy total | PENRE=non-renewable primary energy
ex. raw materials | PENRM=non-renewable primary energy used as raw materials | PENRT=non-renewable primary energy total | SM=use of secondary material | RSF=use of renewable
secondary fuels | NRSF=use of non-renewable secondary fuels | FW=use of net fresh water
ACETube® | ReTHiNK-58059 20 / 25
Environmental Product Declaration
5 Results
OTHER ENVIRONMENTAL INFORMATION DESCRIBING WASTE CATEGORIES
Abbreviation Unit A1 A2 A3 A4 A5 C1 C2 C3 C4 D
HWD Kg 1.61E-5 1.31E-7 1.79E-6 6.34E-6 1.70E-6 0.00E+0 7.62E-7 3.83E-6 1.31E-7 -3.26E-5
NHWD Kg 1.99E-1 3.28E-3 3.51E-2 1.39E-1 4.63E-2 0.00E+0 1.91E-2 4.96E-2 3.44E-1 -1.48E-2
RWD Kg 6.12E-5 3.39E-7 1.25E-5 2.09E-5 5.63E-6 0.00E+0 1.97E-6 7.23E-6 5.12E-7 -1.52E-5
HWD=hazardous waste disposed | NHWD=non hazardous waste disposed | RWD=radioactive waste disposed
ENVIRONMENTAL INFORMATION DESCRIBING OUTPUT FLOWS
Abbreviation Unit A1 A2 A3 A4 A5 C1 C2 C3 C4 D
CRU Kg 0.00E+0 0.00E+0 0.00E+0 0.00E+0 0.00E+0 0.00E+0 0.00E+0 0.00E+0 0.00E+0 0.00E+0
MFR Kg 0.00E+0 0.00E+0 3.05E-3 0.00E+0 5.72E-3 0.00E+0 0.00E+0 6.87E-2 0.00E+0 0.00E+0
MER Kg 0.00E+0 0.00E+0 0.00E+0 0.00E+0 0.00E+0 0.00E+0 0.00E+0 0.00E+0 0.00E+0 0.00E+0
EET MJ 0.00E+0 0.00E+0 5.17E-1 0.00E+0 0.00E+0 0.00E+0 0.00E+0 0.00E+0 0.00E+0 1.12E+1
EEE MJ 0.00E+0 0.00E+0 3.00E-1 0.00E+0 0.00E+0 0.00E+0 0.00E+0 0.00E+0 0.00E+0 6.53E+0
CRU=Components for re-use | MFR=Materials for recycling | MER=Materials for energy recovery | EET=Exported Energy Thermic | EEE=Exported Energy Electric
ACETube® | ReTHiNK-58059 21 / 25
Environmental Product Declaration
5 Results
5.5 INFORMATION ON BIOGENIC CARBON CONTENT PER SQUARE METER
BIOGENIC CARBON CONTENT
The following Information describes the biogenic carbon content in (the main parts of) the
product at the factory gate per square meter:
Biogenic carbon content Amount Unit
Biogenic carbon content in the product 0 kg C
Biogenic carbon content in accompanying packaging 0 kg C
ACETube® | ReTHiNK-58059 22 / 25
Environmental Product Declaration
6 Interpretation of results
As shown in the figure below, the raw material supply (A1) dominates in most
environmental core indicators, often followed by waste processing (C3). The highest
influence on the Global Warming Potential (GWP-total) have raw material supply (A1) and
waste processing (C3). Transports (A2, C2) have rather a minor impact within all core
indicators.
ACETube® | ReTHiNK-58059 23 / 25
Environmental Product Declaration
7 References
ISO 14040
ISO 14040:2006-10, Environmental management - Life cycle assessment - Principles and
framework; EN ISO 14040:2006
ISO 14044
ISO 14044:2006-10, Environmental management - Life cycle assessment - Requirements
and guidelines; EN ISO 14040:2006
ISO 14025
ISO 14025:2011-10: Environmental labels and declarations — Type III environmental
declarations — Principles and procedures
EN 15804+A2
EN 15804+A2: 2019: Sustainability of construction works — Environmental Product
Declarations — Core rules for the product category of construction products
PCR A: General Program Category Rules for Construction Products from the EPD program
Kiwa-Ecobility Experts, 2022-02-14
PCR B: Product Category Rules (PCR) from the Kiwa-Ecobility Experts (Kiwa-EE) – Specific
Product Category Rules: Geosynthetic products, 2023-07-21
ACETube® | ReTHiNK-58059 24 / 25
Environmental Product Declaration
8 Contact information
Publisher Operator Owner of declaration
Kiwa-Ecobility Experts Kiwa-Ecobility Experts Gold-Joint Industry Co., Ltd.
Voltastraße 5 Voltastraße 5 No.33, Jing 3 Rd. Wuqi Dist.
13355 Berlin, DE 13355 Berlin, DE 43541 Taichung City, Taiwan (R.O.C.), TW
E-mail: E-mail: E-mail:
DE.Ecobility.Experts@kiwa.com DE.Ecobility.Experts@kiwa.com marketing@geoace.com
Website: Website: Website:
https://www.kiwa.com/de/en/themes/ecobility-experts/ecobility-https://www.kiwa.com/de/en/themes/ecobility-experts/ecobility-www.geoace.com
experts-epd-program/ experts-epd-program/
Kiwa-Ecobility Experts is
established member of the
ACETube® | ReTHiNK-58059 25 / 25
