ENVIRONMENTAL PRODUCT DECLARATION
as per ISO 14025 and EN 15804+A1
Owner of the Declaration NedZink B.V.
Programme holder Institut Bauen und Umwelt e.V. (IBU)
Publisher Institut Bauen und Umwelt e.V. (IBU)
Declaration number EPD-NED-20200254-IBC1-EN
Issue date 15.06.2021
Valid to 14.06.2026
NedZink NOVA, NedZink NEO, NedZink NOIR
NedZink B.V.
www.ibu-epd.com | https://epd-online.com
Umwelt Produktdeklaration Name des Herstellers – Name des Produkts
1. General Information
NedZink B.V. NedZink® NOVA / NedZink® NEO /
NedZink® NOIR
Programme holder Owner of the declaration
IBU – Institut Bauen und Umwelt e.V. NedZink B.V.
Panoramastr. 1 Hoofdstraat 1
10178 Berlin 6024 AA, Budel-Dorplein
Germany Netherlands
Declaration number Declared product / declared unit
EPD-NED-20200254-IBC1-EN 1kg NedZink® NOVA/NedZink® NEO/NedZink® NOIR,
pre-weathered titanium zinc
This declaration is based on the product Scope:
category rules: The Life Cycle Assessment (LCA) was carried out
Building metals, 11.2017 according to ISO 14040, ISO 14044 and EN 15804.
(PCR checked and approved by the SVR) The LCA is performed for the pre-weathered products
NedZink® NOVA/NedZink® NEO/NedZink® NOIR
manufactured by NedZink B.V. in Budel-Dorplein,
Issue date
Netherlands.
15.06.2021
The pre-weathered rolled zinc from NedZink covered
by this EPD can be used in buildings as roof, façade or
Valid to rainwater systems.
14.06.2026 The LCA was carried out for the manufacturing phase
of the declared product, containing information on raw
and secondary material production, transport and
packaging (cradle to gate). Possible credits after the
end of life phase (module D), waste disposal (C4) and
transport to waste disposal (C2) are also included.
The owner of the declaration shall be liable for the
underlying information and evidence; the IBU shall not
be liable with respect to manufacturer information, life
cycle assessment data and evidences.
The EPD was created according to the specifications
of EN 15804+A1. In the following, the standard will be
simplified as EN 15804.
Verification
The standard EN 15804 serves as the core PCR
Independent verification of the declaration and data
according to ISO 14025:2010
Dipl. Ing. Hans Peters internally x externally
(chairman of Institut Bauen und Umwelt e.V.)
Dr. Alexander Röder Mr Olivier Muller
(Managing Director Institut Bauen und Umwelt e.V.)) (Independent verifier)
2. Product
2.1 Product description/Product definition The defined material properties are checked by an
NedZink® NOVA / NedZink® NEO / NedZink® NOIR is independent and neutral research institute.
pre-weathered titanium zinc produced by NedZink This product certification and the ISO 9001 certificate
according to EN 988. for the quality management system at NedZink assure
Small quantities, as specified in EN 988, of the alloy a constant and uniform high quality standard.
elements copper, titanium and aluminium are added to
electrolytically refined zinc (with a purity of min. NedZink® NOVA is pre-weathered titanium zinc in a
99,995% Zn, Z1 according to EN 1179). matt natural medium grey color. NedZink® NEO is pre-
The chemical composition, mechanical and physical weathered titanium zinc in a matt natural mineral grey
properties and measurement tolerances are color. NedZink® NOIR is pre-weathered titanium zinc
determined in the KOMO product certificate in an anthracite black color.
and certified as NedZink NTZ® by Lloyd's Register
Product certificate (approval No QIS 122).
2 Environmental Product Declaration NedZink B.V. – NedZink NOVA, NedZink NEO, NedZink NOIR
For the placing on the market of the product in the 2.5 Base materials/Ancillary materials
European Union/European Free Trade Association Components of NedZink alloy
(EU/EFTA) (with the exception of Switzerland) The composition of pre-weathered rolled zinc from
Regulation (EU) No. 305/2011 (CPR) applies. The NedZink is in accordance with EN988:
product needs a Declaration of Performance taking - Special-High-Grade zinc 99.995% (Z1 according to
into consideration EN 14782:2006, Self-supporting EN 1179)
metal sheet for roofing, external cladding and internal - Copper: 0.08 - 0.17%
lining, or EN 14783:2013, Fully supported metal sheet - Titanium: 0.07 - 0.12%
and strip for roofing, external cladding and internal - Aluminium: ≤ 0.015%
lining, and the CE-marking. Auxiliary substances
For the application and use the respective national Lubricant oil: 0.89 kg/t zinc; a number of different
provisions apply. agents for cleaning, activating and phosphating;
temporary protection: 1 - 1.5 µm thickness
2.2 Application
NedZink® NOVA / NedZink® NEO / NedZink® NOIR None of the components included in the final product is
titanium zinc coils, sheets, strips and profiles are used listed in the Candidate List of Substances of Very High
for: Concern for Authorisation (SVHC) dated 01/2018.
- roof and façade cladding (CE-marked based on The product does not contain substances with
EN14782:2006, Self-supporting metal sheet for carcinogenic mutagenic reprotoxic (CMR) properties
roofing, external cladding and internal lining or >0.1%.
EN14783:2013, Fully supported metal sheet and strip
for roofing, external cladding and internal lining) 2.6 Manufacture
- interior use The manufacturing process of pre-weathered rolled
- roof drainage systems (gutters, downpipes and zinc includes the following steps:
accessories according to EN612)
- ornaments Pre-alloy:
In order to improve the properties of zinc, and for
2.3 Technical Data energy saving purposes, a pre-alloy with titanium,
The main constructional data are presented in the copper and aluminium is prepared in an induction
following table: furnace. This pre-alloy is poured into ingots.
Constructional data Melting:
Name Value Unit In the melting furnace the Special High Grade (SHG)
Coefficient of thermal expansion 22 10-6K-1 zinc and the ingots are mixed homogeneously. Zinc
Tensile strength ≥ 150 N/mm2 with the right composition is pumped to the casting
not furnace.
Compressive strength N/mm2
relevant
Modulus of elasticity ≥ 80000 N/mm2 Casting:
Melting point 420 °C Casting takes place from the casting furnace into a
Thermal conductivity 110 W/(mK) vertical casting installation. The zinc is cast into blocks,
Electrical conductivity at 20°C 17000000 Ω-1m-1 cooled down with a closed water system and stored for
further processing.
Density 7200 kg/m3
Required testing standards are described in EN 988.
Rolling and coiling:
Blocks coming from the casting installation are
Performance data of the product in accordance with
homogeneous pre-heated for the “hot rolling” process.
the declaration of performance with respect to its
This takes place in a gas-fired continuous oven.
essential characteristics according to EN
During the hot rolling on a reversible rolling machine
14782 and EN 14783 respectively.
the blocks are processed to a predefined thickness. At
the end of the rolling installation the zinc is coiled and
2.4 Delivery status
stored to cool off.
NedZink material is delivered in thicknesses from 0.5
On the reversible cold-rolling mill the coils are rolled to
to 1.5 mm. As average production data is considered,
the desired final thickness. For cooling and lubrication
the LCIA results reflect the environmental profile of
of the process a special emulsion is used
weighted average product thickness: 0.750 mm.
The maximum width of sheets, coils and strips is 1000
Stretching and cutting:
mm.
Tension in the coils is released by a stretching-and
The standard sheets are delivered in 1000 x 2000 mm,
straightening process. The zinc is uniquely marked and
1000 x 2250 mm and 1000 x 3000 mm.
slitted and cut to the desired width and length.
Finished products are delivered to customer
specification.
Pre-weathering:
In a continuously operating production line the coils are
Application rules:
degreased, brushed and phosphated to get a
EN988:1996, Zinc and zinc alloys - Specifications for
prepatinated medium grey appearance for NedZink®
rolled flat products for buildings
NOVA or a mineral grey appearance for NedZink®
EN612:2005, Eaves gutters with bead stiffened fronts
NEO.
and rainwater pipes with seamed joints made of metal
With an additional process for NedZink® NOIR an
sheet.
anthracite black appearance is created. After rinsing
and drying the material surface is provided with a thin
transparent protection layer and stored in the
warehouse.
3 Environmental Product Declaration NedZink B.V. – NedZink NOVA, NedZink NEO, NedZink NOIR
influence of water a zinc-hydroxide is developed. In the
Quality control: final step a reaction with carbon dioxide creates a non-
During the entire process extensive quality checks are water-soluble coating of basic zinc carbonate, being
conducted by the manufacturer and Lloyd's Register. the patina.
Quality Management according to ISO 9001. Therefore NedZink material does not require any
Product quality is checked by Lloyd's Register and maintenance and cleaning during the period of use. If
approved with an Industrial Quality Scheme Approval the surface is slightly damaged, this naturally formed
Certificate QIS122. patina layer will heal itself.
Additionally the quality control is audited by Kiwa and NedZink material is UV-resistant, non-flammable and
certified with KOMO product certificates: resistant to radiating heat. Direct contact with chemical
- BRL2034, K7054/04 zinc sheets substances, especially those containing acids, has to
- BRL2035, K7057/04 zinc gutters be avoided. A list of substances to be avoided can be
- BRL2044, K7063/04 zinc downpipes found on www.nedzink.com.
2.7 Environment and health during The material has a repellent effect to electrosmog
manufacturing (electromagnetic radiation) and the effects of rain and
The manufacturing process is carried out according to snow may be neglected.
the rules as laid down in the environmental permit.
NedZink’s policy follows the Total Quality Management 2.11 Environment and health during use
(TQM). Environment
The directives of the Environmental Management The due to air and water formed patina (zinc
System ISO14001 are an integral part of the Quality carbonate) is a natural protection layer. Due to this
Management System ISO9001. patina the transfer of zinc ions via rain water is
constantly reduced, because this protection layer is
2.8 Product processing/Installation non-water-soluble.
Basic principles: Further transfer of zinc ions is mainly related to the air
NedZink material must be stored under dry and pollution with SO . Due to the reduction of SO
2 2
ventilated conditions. This applies storage in concentration in the air, the zinc-concentration of
warehouses, on building sites, on installation sites as precipitation in the rainwater has subsequently been
well as during transportation. Coils are to be stored on reduced to one fifth of the former values during the last
their original pallets. thirty years.
Transportation should only be done in enclosed As a result of all environmental regulations this amount
vehicles. will reduce even more in the future, due to the
Temperature deviations have to be avoided as it can reduction of SO concentration in the air.
2
result in varying humidity levels. The transfer of zinc ions via rain water is constantly
All contact between zinc and moisture (wet surface, reduced due to developing a natural protection layer of
rain or dew) during handling and transportation must zinc carbonate.
be avoided. Wet surfaces (with or without protective
film) may not directly be covered. In aquatic systems only a small part of the total zinc
concentration is available for organisms (bioavailable).
The material is to be processed without tension. It is related to the physical-chemical conditions of the
receiving water body.
The thermal expansion has to be taken into account
when installing/handling the product. Health
When used according to their designated function,
Mechanical deformation of zinc should be avoided in NedZink products will have no health effects.
case the zinc temperature is not at least 7°C. Zinc is an essential metal, necessary for living
organisms. Zinc does not accumulate in the body.
Further installation rules are listed on The recommended daily intake of zinc (in the correct
www.nedzink.com. form) according to the WHO 15mg/day for men and
12mg/day for women.
2.9 Packaging
The packaging material in use are wooden pallets, 2.12 Reference service life
paper/cardboard and plastics (films and wires). All The service life depends on the correct application
packaging materials are reusable and/or recyclable, if according to the guidelines for processing and
gathered separately. installation. The theoretical lifetime according to the
The take-back and recycling of our packaging in available literature is > 100 years.
Germany is organized by Interseroh. Service lifetime according to Bundesinstitut für Bau-
Stadt- und Raumforschung (BBSR): > 50 years.
As the EPD scope is a cradle-to-gate with options, no
2.10 Condition of use reference service life is declared in the LCA.
NedZink material develops a protective patina layer, The standard ISO 15686 has not been considered.
which darkens the material slightly over time due to a
reaction with oxygen and carbon dioxide (air and
water). 2.13 Extraordinary effects
This layer is responsible for the high resistance of
titanium zinc against corrosion. For both pre- Fire
weathered zinc and natural rolled zinc this behavior is The NedZink® products comply with EN13501-1: the
the same. requirements of building material Class A1 "non-
Zinc in contact with air creates a zinc-oxide. Due to the combustible". (96/603/EC)
4 Environmental Product Declaration NedZink B.V. – NedZink NOVA, NedZink NEO, NedZink NOIR
from other materials. Zinc can then easlily be collected
Fire protection for re-use and/or recycling.
Name Value
Building material class EN13501 Re-use/Recycling:
A1
DIN4102 Scrap produced during the manufacturing process
Burning droplets EN13501 D0 from NedZink material are 100% remelted and fed
Smoke gas development back completely into NedZink's production process. A
-
EN13501 small amount of residue (skimmings, dross, dust),
which is no longer valuable for the internal production
Smoke production process, is completely recycled by a third party
Vaporization as zinc oxide (ZnO) occurs when heated (European Waste Code 10.05.01).
above 650 °C. The produced ZnO smoke may cause
zinc fever (diarrhoea, dry throat, feverish) when The scrap from demolition and renovation work on
inhaled over some (period of) time. The effects building sites is collected and sold either directly to
disappear completely in 1 to 2 days after the secondary smelting works or via a scrap metal dealer.
inhalation. The recycling rate for zinc sheets is over 95%. Credits
for this recycling are appointed in module D. These
Water credits are based on a recycling percentage of 95%
Zinc is not classified as hazardous for the aquatic (European recycling rate for rolled zinc).
environment.
2.15 Disposal
Mechanical destruction Due to the effective recycling process, a maximum of
Given the metallic nature of the product, there will be 5% zinc has to be disposed.
no environmental effect. The European Waste Code for collected zinc after
disassembly is 17.04.04.
2.14 Re-use phase
Disassembly: 2.16 Further information
During disassembly of a building construction or Additional information, optional details, references,
renovations NedZink material should be separated data sheets can be obtained at: www.nedzink.com
3. LCA: Calculation rules
3.1 Declared Unit
The declared unit is 1 kg of NedZink® NOVA / 3.5 Background data
NedZink® NEO / NedZink® NOIR, pre-weathered Background processes are taken from the Ecoinvent
titanium zinc. V3.6 database, (2019), with the “allocation, cut-off by
classification” system model.
Declared unit Life cycle inventory data for the production of zinc
Name Value Unit concentrate and SHG Zinc in the Ecoinvent V3.6
Declared unit 1 kg database is updated with the most recent LCA report
conversion factor [Mass/Declared (Zinc Environmental Profile - 2015 Update) on primary
1 -
Unit] Zinc by the International Zinc Association.
Gross density 7200 kg/m3 The environmental impact of the SHG Zinc was then
calculated using SimaPro V9.0. Site-specific data was
provided by NedZink and verified against earlier
studies.
3.2 System boundary
Type of the EPD: Cradle-to-Gate with options. Modules 3.6 Data quality
A1, A2 and A3 contain information on the raw- and The data used for this study was both of high quality
secondary material extraction, transport to the and recent. The specific data was collected by the
manufacturer, manufacturing and packaging. manufacturer, The generic data that is used is less
Only the transport to module C4 is considered under than 10 years old or has been updated within this
module C2. Module C4 takes into account the non- period. This is in compliance with the data quality
recovered zinc at the end of life. Modules A4, A5, B1- requirements of EN 15804.
B7, C1 and C3 are not declared.
Credits after End-of-Life of the product are also 3.7 Period under review
included (module D). Site-specific data for the year 2019 and 2020 was used
in this study. Background data is taken from the
3.3 Estimates and assumptions Ecoinvent V3.6 database (2019) and varies in age.
No major estimates or assumptions were required for
the creation of this EPD. 3.8 Allocation
Allocation was avoided as much as possible in this
3.4 Cut-off criteria study, as required in EN 15804.
No major cut-offs were applied to specific However, the following allocation had to be done:
manufacturing data from Nedzink. Production impacts - For pre-weathered zinc, there is a net output stream
of packaging for raw materials are not known and of rejected zinc product to internal recycling. As this is
excluded, waste processing of this packaging is known an internal recycling process, 0 impacts are allocated
and included. For upstream data a background to this material flow.
database (Ecoinvent V3.6) was used, which can
contain additional cut-offs.
5 Environmental Product Declaration NedZink B.V. – NedZink NOVA, NedZink NEO, NedZink NOIR
3.9 Comparability context, respectively the product-specific
Basically, a comparison or an evaluation of EPD data characteristics of performance, are taken into account.
is only possible if all the data sets to be compared
were created according to EN 15804 and the building
4. LCA: Scenarios and additional technical information
Modules A4, A5, B1-B7 C1 and C3 are not considered
in this study. The possible credits given in Module D
are based on 100% recyclability of zinc products. After
the collection (a collection rate of 95% is taken), zinc
scrap is re-melted and converted to secondary zinc.
This is not done by NedZink but by third parties. The
possible credit for the zinc gained through re-melting is
calculated using the dataset of the primary zinc
production. The remaining zinc (5%) is landfilled
(module C4).
End of life (C4) / Recycling potentials (D)
Name Value Unit
Recycling 95% kg
Landfilling 5% kg
6 Environmental Product Declaration NedZink B.V. – NedZink NOVA, NedZink NEO, NedZink NOIR
5. LCA: Results
DESCRIPTION OF THE SYSTEM BOUNDARY (X = INCLUDED IN LCA; MND = MODULE NOT DECLARED;
MNR = MODULE NOT RELEVANT)
BENEFITS AND
CONSTRUCTI LOADS
PRODUCT STAGE ON PROCESS USE STAGE END OF LIFE STAGE BEYOND THE
STAGE SYSTEM
BOUNDARIES
7 Environmental Product Declaration NedZink B.V. – NedZink NOVA, NedZink NEO, NedZink NOIR
lairetam
waR
ylppus tropsnarT
gnirutcafunaM
eht
morf
tropsnarT
etis
eht
ot
etag
ylbmessA esU
ecnanetniaM
riapeR
tnemecalpeR tnemhsibrufeR
ygrene
lanoitarepO esu
retaw
lanoitarepO esu
noitcurtsnoc-eD
noitilomed tropsnarT
gnissecorp
etsaW
lasopsiD -esueR -yrevoceR -gnilcyceR laitnetop
A1 A2 A3 A4 A5 B1 B2 B3 B4 B5 B6 B7 C1 C2 C3 C4 D
X X X MND MND MND MND MNR MNR MNR MND MND MND X MND X X
RESULTS OF THE LCA - ENVIRONMENTAL IMPACT according to EN 15804+A1: 1 kg NEDZINK
NOVA/NEO/NOIR
Parameter Unit A1-A3 C2 C4 D
Global warming potential [kg CO2-Eq.] 4.53E+0 6.52E-4 2.58E-4 -2.77E+0
Depletion potential of the stratospheric ozone layer [kg CFC11-Eq.] 3.59E-7 1.21E-10 8.61E-11 -2.07E-7
Acidification potential of land and water [kg SO2-Eq.] 3.58E-2 2.81E-6 1.89E-6 -2.22E-2
Eutrophication potential [kg (PO4)3--Eq.] 4.55E-3 5.18E-7 3.33E-7 -3.18E-3
Formation potential of tropospheric ozone photochemical
[kg ethene-Eq.] 1.28E-3 9.39E-8 7.92E-8 -7.24E-4
oxidants
Abiotic depletion potential for non-fossil resources [kg Sb-Eq.] 9.30E-2 1.70E-8 2.41E-9 -7.32E-2
Abiotic depletion potential for fossil resources [MJ] 5.29E+1 9.89E-3 7.28E-3 -3.10E+1
RESULTS OF THE LCA - INDICATORS TO DESCRIBE RESOURCE USE according to EN 15804+A1: 1 kg
NEDZINK NOVA/NEO/NOIR
Parameter Unit A1-A3 C2 C4 D
Renewable primary energy as energy carrier [MJ] 8.73E+0 1.45E-4 5.95E-5 -5.62E+0
Renewable primary energy resources as material utilization [MJ] 2.01E-1 0.00E+0 0.00E+0 0.00E+0
Total use of renewable primary energy resources [MJ] 8.93E+0 1.45E-4 5.95E-5 -5.62E+0
Non-renewable primary energy as energy carrier [MJ] 7.14E+1 1.07E-2 7.82E-3 -4.40E+1
Non-renewable primary energy as material utilization [MJ] 0.00E+0 0.00E+0 0.00E+0 0.00E+0
Total use of non-renewable primary energy resources [MJ] 7.14E+1 1.07E-2 7.82E-3 -4.40E+1
Use of secondary material [kg] 0.00E+0 0.00E+0 0.00E+0 9.47E-1
Use of renewable secondary fuels [MJ] 0.00E+0 0.00E+0 0.00E+0 0.00E+0
Use of non-renewable secondary fuels [MJ] 0.00E+0 0.00E+0 0.00E+0 0.00E+0
Use of net fresh water [m³] 1.20E-1 1.14E-6 7.86E-6 -8.95E-2
RESULTS OF THE LCA – WASTE CATEGORIES AND OUTPUT FLOWS according to EN 15804+A1:
1 kg NEDZINK NOVA/NEO/NOIR
Parameter Unit A1-A3 C2 C4 D
Hazardous waste disposed [kg] 1.18E-2 2.58E-8 1.10E-8 -9.46E-3
Non-hazardous waste disposed [kg] 6.39E-1 6.26E-4 5.00E-2 -4.08E-1
Radioactive waste disposed [kg] 3.06E-4 6.87E-8 4.83E-8 -2.14E-4
Components for re-use [kg] 0.00E+0 0.00E+0 0.00E+0 0.00E+0
Materials for recycling [kg] 1.88E-1 0.00E+0 0.00E+0 0.00E+0
Materials for energy recovery [kg] 0.00E+0 0.00E+0 0.00E+0 0.00E+0
Exported electrical energy [MJ] 0.00E+0 0.00E+0 0.00E+0 0.00E+0
Exported thermal energy [MJ] 0.00E+0 0.00E+0 0.00E+0 0.00E+0
6. LCA: Interpretation
The 7 main impact categories for 1 kg of Nedzink The remaining contributions mainly consist of energy
Nova, Neo, Noir usage (electricity and gas), substances used for pre-
weathering and a small contribution from the remaining
Life cycle inventory data for the production of zinc metal components (Cu, Ti, Al).
concentrate and Special High Grade Zinc (SHG Zinc)
in the background database Ecoinvent V3.6 is aligned Because of the high contribution of SHG Zinc and the
with data from the IZA 2015 LCA report (Zinc high recyclability that is assumed, the amount of
Environmetal Profile - 2015 Update, see also section credits gained in module D for each impact category is
3.5 Background Data). high, at least 57% or higher compared to the initial
impact value.
The contribution of SHG Zinc is the dominating factor
in all of the impact categories, with contributions >70%
in for all indicators.
7. Requisite evidence
In a literature study TNO-MEP-99/441 of TNO (Dutch The run-off rate is influenced by the atmospheric
Organisation for Applied Scientific Research) the conditions, of which the SO2 concentration is the most
emissions from corrosion of zinc to water have been important variable. With the decreasing of the SO2
evaluated. This corrosion rate refers to the loss of concentration, the corrosion rate is also decreasing.
metallic zinc.
The run-off rate is the wash-off of zinc from the patina In areas with higher SO2-concentration a run-off rate
layer. This run-off rate is generally lower than the off 3 g/m2.yr can be calculated and 2 g/m2.yr in areas
corrosion rate. with lower concentration.
During the built up of the zinc patina layer the run-off is
lower than the corrosion rate. The growth of the patina
layer delays the corrosion.
8. References
General Programme Instructions
Institut Bauen und Umwelt e.V., Berlin (pub.): The PCR 2017 Part B
preparation of environmental product declarations Institut Bauen und Umwelt e.V., Berlin: Product
(EPDs); General Programme Instructions for the Category Rules for Construction Products from the
preparation of EPDs at the Institut Bauen und Umwelt range of Environmental Product Declarations of Institut
e.V. (IBU), 2016/03 Bauen und Umwelt (IBU), Part B: Requirements on the
www.ibu-epd.com EPD for Building Metals. Version 1.6, November 2017
www.ibu-epd.com
PCR 2017 Part A EN 988
Institut Bauen und Umwelt e.V., Berlin: Product EN 988:1996
Category Rules for Construction Products from the Zinc and zinc alloys - Specification for rolled flat
range of Environmental Product Declarations of Institut products for building
Bauen und Umwelt (IBU), Part A: Calculation Rules for
the Life Cycle Assessment and Requirements on the EN 1179
Background Report. Version 1.8, July 2019 EN 1179:2003
www.ibu-epd.com Zinc and zinc alloys - Primary zinc
8 Environmental Product Declaration NedZink B.V. – NedZink NOVA, NedZink NEO, NedZink NOIR
ISO 14044
EN 612 ISO 14044:2006
EN 612:2005 Environmental management - Life cycle assessment -
Eaves gutters with bead stiffened fronts and rainwater Requirements and guidelines
pipes with seamed joints made of metal sheet
ISO 15686
EN 13501-1 ISO 15686
EN 13501-1:2007+A1:2009 Buildings and constructed assets - Service life
Fire classification of construction products and building planning
elements - Part 1: Classification using data from
reaction to fire tests 96/603/EC
EU Commission Decision of 4 October 1996
EN 13501-5 establishing the list of products belonging to Classes A
EN 13501-5:2006+A1:2009 'No contribution to fire' provided for in Decision
Fire classification of construction products and building 94/611/EC implementing Article 20 of Council Directive
elements - Part 5: Classification using data from 89/106/EEC on construction products (Text with EEA
external fire exposure to roofs tests relevance)
EN 14782 KOMO product certificates
EN 14782:2006 BRL2034: K7054/04 zinc sheets
Self-supporting metal sheet for roofing, external BRL2035: K7057/04 zinc gutters
cladding and internal lining - Product specification and BRL2044: K7063/04 zinc downpipes
requirements
Lloyd's Register Product certificate (approval No
EN 14783 QIS 122)
EN 14783:2013 Lloyd’s Register Inspection Services - Product
Fully supported metal sheet and strip for roofing, certificate Industrial Quality Scheme for Product
external cladding and internal lining - Product Certification by Surveillance of Quality Systems
specification and requirements (approval No QIS 122)
EN 15804 Candidate List of substances of very high concern
EN 15804:2012-04+A1:2013 for Authorisation
Sustainability of construction works - Environmental ECHA published in accordance with Article 59(10) of
Product Declarations - Core rules for the product the REACH Regulation (2018)
category of construction products
TNO-MEP-99/441
DIN 4102 Diffusive Emissions of zinc due to atmospheric
DIN 4102 corrosion of zinc and zinc coated (galvanised)
Fire behaviour of building materials and building materials - R.H.J. Korenromp, J.C.Th. Hollander
components (1999)
ISO 9001 Zinc Environmental Profile - 2015 Update
ISO 9001:2015 International Zinc Association (2016)
Quality management systems - Requirements
Zinc Recycling, Closing the Loop
ISO 14001 International Zinc Association (2011)
ISO 14001:2015
Environmental management systems - Requirements Zinc…A Sustainable Material
with guidance for use International Zinc Association (2010)
ISO 14025 Zinc, A Sustainable Material – Essential for Modern
ISO 14025:2011-10 Life.
Environmental labels and declarations - Type III International Zinc Association (2017)
environmental declarations - Principles and procedures
SimaPro V9.0
ISO 14040 Life Cycle Assessment software
ISO 14040:2006
Environmental management - Life cycle assessment - Ecoinvent V3.6
Principles and framework Life Cycle Inventory database, 2019
9 Environmental Product Declaration NedZink B.V. – NedZink NOVA, NedZink NEO, NedZink NOIR
Publisher
Institut Bauen und Umwelt e.V. Tel +49 (0)30 3087748- 0
Panoramastr. 1 Fax +49 (0)30 3087748- 29
10178 Berlin Mail info@ibu-epd.com
Germany Web www.ibu-epd.com
Programme holder
Institut Bauen und Umwelt e.V. Tel +49 (0)30 - 3087748- 0
Panoramastr 1 Fax +49 (0)30 – 3087748 - 29
10178 Berlin Mail info@ibu-epd.com
Germany Web www.ibu-epd.com
Author of the Life Cycle
Assessment Tel +31 (0)30-693 00 55
Stichting Adviescentrum Metaal Fax +31 (0)30-693 00 57
Kelvinbaan 40 Mail info@metaaladvies.nl
3430MT Nieuwegein Web metaaladvies.nl
Netherlands
Owner of the Declaration
NedZink B.V. Tel +31 (0)475 455700
Hoofdstraat 1 Fax +31 (0)475 455790
6024AA Budel-Dorplein Mail info@nedzink.com
Netherlands Web www.nedzink.com
