ENVIRONMENTAL PRODUCT DECLARATION
as per ISO 14025 and EN 15804+A2
Owner of the Declaration Sika Schweiz AG
Publisher Institut Bauen und Umwelt e.V. (IBU)
Programme holder Institut Bauen und Umwelt e.V. (IBU)
Declaration number EPD-SIK-20240173-CBA2-EN
Issue date 20/06/2024
Valid to 19/06/2029
Sika® ViscoCrete®-4097
Sika Schweiz AG
www.ibu-epd.com | https://epd-online.com
General Information
Sika Schweiz AG Sika® ViscoCrete®-4097
Programme holder Owner of the declaration
IBU – Institut Bauen und Umwelt e.V. Sika Schweiz AG
Hegelplatz 1 Tüffenwies 16
10117 Berlin 8048 Zürich
Germany Switzerland
Declaration number Declared product / declared unit
EPD-SIK-20240173-CBA2-EN 1 kg of Sika® ViscoCrete®-4097 with a density of 1.08 g/ml
This declaration is based on the product category rules: Scope:
Concrete admixtures, 01/08/2021 This core-EPD relates to 1 kg of Sika® ViscoCrete®-4097 with a density of
(PCR checked and approved by the SVR) 1.08 g/ml, a high-performance superplasticizer, produced in Kirchberg,
Switzerland and is representative for the year 2022.
Issue date The results in this core-EPD were calculated using an LCA-tool verified by
IBU in 2023.
20/06/2024
The owner of the declaration shall be liable for the underlying information
and evidence; the IBU shall not be liable with respect to manufacturer
Valid to
information, life cycle assessment data and evidences.
19/06/2029
The EPD was created according to the specifications of EN 15804+A2. In
the following, the standard will be simplified as EN 15804.
Verification
The standard EN 15804 serves as the core PCR
Independent verification of the declaration and data according to ISO
14025:2011
internally X externally
Dipl.-Ing. Hans Peters
(Chairman of Institut Bauen und Umwelt e.V.)
Florian Pronold Matthias Schulz,
(Managing Director Institut Bauen und Umwelt e.V.) (Independent verifier)
1 Environmental Product Declaration - Sika Schweiz AG - Sika® ViscoCrete®-4097
Product
Name Value Unit
Product description/Product definition
~
Sika® ViscoCrete®-4097 is a high range water reducing Solids content (SN EN 480-8) M.-%
34.7
admixture utilizing Sika's ViscoCrete polycarboxylate
pH value (ISO 4316) ~ 4.8
technology. Sika® ViscoCrete®-4097 meets the requirements of
~
SN EN 934-2: plasticizer for concrete. Specific Gravity (ISO 758) g/cm3
1.08
Sika® ViscoCrete®-4097 is designed for use in Chloride content (SN EN 480-10) ≤ 0.1 M.-%
▪ Recycled concrete RC-C, RC-M Alkali content (SN EN 480-12) ≤ 1.0 M.-%
▪ Concrete with highly absorbent aggregate granulation Air content of fresh concrete (EN 12350-7) 1.3 Vol.-%
▪ With increased coarse air in the fresh concrete
Water reduction (SN EN 12350-5) + 250 mm
▪ Concrete with long transport distances
1 day Compressive strength at equal
▪ At elevated temperatures 29.9 N/mm2
consistence (SN EN 12390-3)
▪ Pumped concrete
28 day Compressive strength at equal
▪ Self-compacting concrete SCC 63.0 N/mm2
consistence (SN EN 12390-3)
▪ Exposed concrete
▪ Concrete with maximum water reduction 28 day Compressive strength at equal water/ 45.6 N/mm2
▪ Waterproof concrete (white tank) cement ratio (SN EN 12390-3)
Increasing consistence (SN EN 12350-5) 600 mm
This all-season additive has the advantage of
Additional technical data are not relevant for this product.
▪ Highest water reduction
Performance data of the product in accordance with the
▪ Highest consistency maintenance
declaration of performance with respect to its essential
▪ Reduced coarse air in fresh concrete
characteristics according to EN 934-2:2009+A1:2012,
▪ Good flowability
Admixtures for concrete, mortar and grout – Part 2: Concrete
▪ High impermeabilities and strengths
admixtures – Definitions, requirements, conformity, marking and
▪ Improved creep and shrinkage behavior
labelling.
▪ Improved durability
▪ Harmless for reinforced and prestressed concrete structures
Base materials/Ancillary materials
For the purposes of this EPD, Sika's Industrie Neuhof 9, 3422
The raw materials and additives of Sika® ViscoCrete®-4097
Kirchberg, Switzerland manufacturing site was selected. The
can be given as follows:
product needs a declaration of performance taking into
consideration SN EN 934-2+A1, Admixtures for concrete,
• Water: 60 – 75%
mortar and grout – Part 2: Concrete admixtures – Definitions,
• Polycarboxylate: 25 – 35%
requirements, conformity, marking and labelling and the CE-
• Additives: 0.5 - 5%
marking. For the application and use the respective national
provisions apply.
Defoaming agents and preservatives are added as minor
Application components and auxiliaries. Sika® ViscoCrete®-4097 is a non-
Sika® ViscoCrete®-4097 is used as a constituent material to chloride-based admixture, it does not contain any intentionally
added chlorides.
produce concrete. It can be used in combination with other Sika
admixtures and can be successfully used in mix designs
This product contains substances listed in the candidate list
utilizing supplementary cementitious materials.
(date: 20.04.2023) exceeding 0.1 percentage by mass: No
Technical Data
Sika® ViscoCrete®-4097 meets the requirements of SN EN This product contains other CMR substances in categories 1A
or 1B which are not on the candidate list, exceeding 0.1
934-2+A1 as superplasticizer.
percentage by mass: No
Constructional data
Biocide products were added to this construction product or it
has been treated with biocide products (this then concerns a
treated product as defined by the (EU) Ordinance on Biocide
Products No. 528/2012): Yes.
Small volumes (< 0.5% by mass) of biocides with functional
chemical groups for example isothiazolinones are used as
preservatives in concrete admixtures during storage. More
detailed information is available in the respective
manufacturer's documentation (e.g. product data sheets, safety
data sheets).
Reference service life
The durability of concreate admixtures is normally at least as
long as the lifetime of the building in which it is used. The
experimental data show that the reference life is greater than
50 years.
2 Environmental Product Declaration - Sika Schweiz AG - Sika® ViscoCrete®-4097
The documentation of the RSL is not required for the EPDs lifecycle is not declared. Only modules A1-A3, A4, A5, C1-C4
calculated using the EPD tool from Sika since the entire and D are considered.
LCA: Calculation rules
The building deconstruction (demolition process) takes place in
Declared Unit C1 module which considers energy production and
The EPD refers to the declared unit of 1 kg of concrete consumption in terms of diesel and all the emissions connected
admixture (superplasticizer) applied into the building with a with the fuel-burning process. After the demolition, the
density of 1.08 g/ml in accordance with IBU PCR 04-2023 part admixture is transported to the end-of-life processing (C2
B for concrete admixtures. module) where all the impacts related to the transport
Declared unit and mass reference processes are considered.
Name Value Unit
One scenario is considered for the final treatment of the waste:
Declared unit 1 kg
Gross density 1080 kg/m3 • 100% disposal (C4), modelled by landfill process
whereadmixtures end their life cycle.
Other declared units are allowed if the conversion is shown
transparently.
Module D accounts for benefits that are beyond the defined
system boundaries. Credits are generated during the
System boundary incineration of the installation scrap in module A5.
Declaration type with respect to life cycle stages covered
Geographic Representativeness
according to clause 5.2 EN 15804+A2 is cradle to gate
Land or region, in which the declared product system is
withmodules C1–C4 and module D (A1–A3, A4, A5, C and D).
manufactured, used or handled at the end of the product´s
Modules taken into account:
lifespan: Switzerland
• A1 Production of preliminary products
• A2 Transport to the plant
Comparability
• A3 Production including provision of energy, production of
Basically, a comparison or an evaluation of EPD data is only
auxiliaries and consumables and waste treatment
possible if all the data sets to be compared were created
• A4 Transport from the construction site to the installation site
according to EN 15804 and the building context, respectively
• A5 Installation, admixtures applied into the building during A5
the product-specific characteristics of performance, are taken
phase operations. At this stage, an impact ofthe production and
into account. Sphera LCA for Expert software (version 10) and
treatment of installation residueequal to 1% of the product is
Managed LCA Content (2022.2) have been used.
considered.
LCA: Scenarios and additional technical information
Material loss regards the amount of product not used during the
Characteristic product properties of biogenic carbon application phase into the building. This amount is 1 % of the
No biogenic carbon is contained in the product or in the product, impacts related to the production of this part
packaging. 75% of Sika® ViscoCrete®-4097 is delivered to arecharged to the A5 module. This percentage is considered
customer as bulk. 25% is delivered by IBCs. IBCs are made of aswaste to incineration since the product has a calorific value
PE-HD and steel. and impacts of its end of life have been considered in the LCA
model and declared in A5.
Information on describing the biogenic carbon content at
factory gate
A reference service life according to the ISO 15686:1, -2, -7
Name ValueUnit
and -8 standards cannot be declared as the additives are fully
kg integrated into mortar/concrete. Their service life thus depends
Biogenic carbon content in product -
C on the service life of the concrete structure they are used in.
Biogenic carbon content in accompanying kg
- End of life (C1-C4)
packaging C
C1: This module considers the use of machinery (7.5E-5 kg of
Note: 1 kg of biogenic carbon is equivalent to 44/12 kg of CO . diesel for kg handled) to dismantle the product to enable its
2
subsequent transport.
C2: The concrete demolition waste is transported from the
building site to a treatment plant or disposal site by truck and
an average distance of 50 km is considered.
Transport from the gate to the site (A4)
C4: The results for the end-of-life are declared for one scenario:
Name Value Unit
Name Value Unit
Transport distance 70 km
Landfill percentage 100 %
Gross weigth 34-40 t
Material to landfill 1 kg
Payload capacity 27 t
Assembly (A5)
Name Value Unit
Material loss 0.01 kg
3 Environmental Product Declaration - Sika Schweiz AG - Sika® ViscoCrete®-4097
LCA: Results
DESCRIPTION OF THE SYSTEM BOUNDARY (X = INCLUDED IN LCA; MND = MODULE OR INDICATOR NOT DECLARED; MNR
= MODULE NOT RELEVANT)
Benefits and
Construction loads beyond
Product stage Use stage End of life stage
process stage the system
boundaries
la ire ta m w a Ry lp p u s tro p s n a rT g n iru tc a fu n a M e h t m o rf tro p s n a rTe tis e h t o t e ta g y lb m e s s A e s U e c n a n e tn ia M ria p e R tn e m e c a lp e R tn e m h s ib ru fe R y g re n e la n o ita re p Oe s u re ta w la n o ita re p Oe s u n o itc u rts n o c -e Dn o itilo m e d tro p s n a rT g n is s e c o rp e ts a W la s o p s iD -e s u e R-y re v o c e R-g n ilc y c e Rla itn e to p
A1 A2 A3 A4 A5 B1 B2 B3 B4 B5 B6 B7 C1 C2 C3 C4 D
X X X X X MND MND MNR MNR MNR MND MND X X MND X X
RESULTS OF THE LCA - ENVIRONMENTAL IMPACT according to EN 15804+A2: 1 kg Sika® ViscoCrete®-4097
Parameter Unit A1-A3 A4 A5 C1 C2 C4 D
GWP-total kg CO 2 eq 1.02E+00 3.72E-03 2.1E-01 2.83E-04 6.27E-03 1.45E-02 -9.19E-02
GWP-fossil kg CO 2 eq 1E+00 3.56E-03 2.05E-01 2.7E-04 6E-03 1.49E-02 -9.15E-02
GWP-biogenic kg CO 2 eq 1.03E-02 1.61E-04 5.23E-03 1.23E-05 2.71E-04 -4.42E-04 -4.68E-04
GWP-luluc kg CO 2 eq 3.15E-03 1.62E-07 3.27E-05 1.25E-08 2.72E-07 2.75E-05 -1.01E-05
ODP kg CFC11 eq 1.82E-12 3.65E-16 3.45E-14 2.82E-17 6.15E-16 3.51E-14 -6.19E-13
AP mol H+ eq 2.36E-03 1.04E-05 1.44E-04 3.62E-06 1.91E-05 1.06E-04 -1.2E-04
EP-freshwater kg P eq 8.56E-06 8.32E-10 5.15E-08 6.41E-11 1.4E-09 2.53E-08 -1.26E-07
EP-marine kg N eq 7.29E-04 4.78E-06 2.11E-05 1.65E-06 8.89E-06 2.71E-05 -3.27E-05
EP-terrestrial mol N eq 8.2E-03 5.25E-05 3.22E-04 1.81E-05 9.78E-05 2.97E-04 -3.5E-04
kg NMVOC
POCP 2.18E-03 9.64E-06 7.15E-05 4.95E-06 1.77E-05 8.22E-05 -9.14E-05
eq
ADPE kg Sb eq 9.42E-07 1.87E-10 2.8E-09 1.44E-11 3.14E-10 1.53E-09 -1.38E-08
ADPF MJ 2.66E+01 4.98E-02 4.05E-01 3.84E-03 8.39E-02 1.95E-01 -1.56E+00
m3 world eq
WDP 3.12E-01 9.63E-06 2.2E-02 7.43E-07 1.62E-05 1.64E-03 -9.75E-03
deprived
GWP = Global warming potential; ODP = Depletion potential of the stratospheric ozone layer; AP = Acidification potential of land and water; EP =
Eutrophication potential; POCP = Formation potential of tropospheric ozone photochemical oxidants; ADPE = Abiotic depletion potential for non-fossil
resources; ADPF = Abiotic depletion potential for fossil resources; WDP = Water (user) deprivation potential)
RESULTS OF THE LCA - INDICATORS TO DESCRIBE RESOURCE USE according to EN 15804+A2: 1 kg Sika® ViscoCrete®-
4097
Parameter Unit A1-A3 A4 A5 C1 C2 C4 D
PERE MJ 1.98E+00 3.02E-04 2.99E-02 2.33E-05 5.08E-04 2.93E-02 -4.28E-01
PERM MJ 0 0 0 0 0 0 0
PERT MJ 1.98E+00 3.02E-04 2.99E-02 2.33E-05 5.08E-04 2.93E-02 -4.28E-01
PENRE MJ 1.96E+01 5E-02 2.98E+00 3.86E-03 8.42E-02 1.96E-01 -1.56E+00
PENRM MJ 7.39E+00 0 -2.57E+00 0 0 0 0
PENRT MJ 2.7E+01 5E-02 4.06E-01 3.86E-03 8.42E-02 1.96E-01 -1.56E+00
SM kg 0 0 0 0 0 0 0
RSF MJ 0 0 0 0 0 0 0
NRSF MJ 0 0 0 0 0 0 0
FW m3 1.05E-02 4.1E-07 5.36E-04 3.16E-08 6.9E-07 4.97E-05 -4.11E-04
PERE = Use of renewable primary energy excluding renewable primary energy resources used as raw materials; PERM = Use of renewable primary
energy resources used as raw materials; PERT = Total use of renewable primary energy resources; PENRE = Use of non-renewable primary energy
excluding non-renewable primary energy resources used as raw materials; PENRM = Use of non-renewable primary energy resources used as raw
materials; PENRT = Total use of non-renewable primary energy resources; SM = Use of secondary material; RSF = Use of renewable secondary fuels;
NRSF = Use of non-renewable secondary fuels; FW = Use of net fresh water
RESULTS OF THE LCA – WASTE CATEGORIES AND OUTPUT FLOWS according to EN 15804+A2:
1 kg Sika® ViscoCrete®-4097
Parameter Unit A1-A3 A4 A5 C1 C2 C4 D
HWD kg 1.46E-09 1.73E-13 1.79E-11 1.33E-14 2.91E-13 1.01E-11 -2.11E-10
NHWD kg 3.85E-02 5.11E-06 2E-03 3.94E-07 8.6E-06 1E+00 -7.86E-04
RWD kg 4.85E-04 8.25E-08 5.76E-06 6.36E-09 1.39E-07 2.18E-06 -1.23E-04
CRU kg 0 0 0 0 0 0 0
MFR kg 0 0 0 0 0 0 0
MER kg 0 0 0 0 0 0 0
EEE MJ 0 0 4.12E-01 0 0 0 0
EET MJ 0 0 7.38E-01 0 0 0 0
4 Environmental Product Declaration - Sika Schweiz AG - Sika® ViscoCrete®-4097
HWD = Hazardous waste disposed; NHWD = Non-hazardous waste disposed; RWD = Radioactive waste disposed; CRU = Components for re-use;
MFR = Materials for recycling; MER = Materials for energy recovery; EEE = Exported electrical energy; EET = Exported thermal energy
RESULTS OF THE LCA – additional impact categories according to EN 15804+A2-optional:
1 kg Sika® ViscoCrete®-4097
Parameter Unit A1-A3 A4 A5 C1 C2 C4 D
Disease
PM 2.05E-08 5.95E-11 1.07E-09 1.93E-10 1.06E-10 1.3E-09 -9.97E-10
incidence
IR kBq U235 eq 5.47E-02 1.24E-05 8.39E-04 9.55E-07 2.08E-05 2.42E-04 -2.08E-02
ETP-fw CTUe 1.15E+01 3.55E-02 2.83E-01 2.74E-03 5.97E-02 1.1E-01 -3.42E-01
HTP-c CTUh 9.36E-10 6.6E-13 7.58E-12 5.09E-14 1.11E-12 1.67E-11 -1.57E-11
HTP-nc CTUh 9.16E-08 3.24E-11 2.81E-10 3.52E-12 5.51E-11 1.85E-09 -6.03E-10
SQP SQP 5.83E+00 2.96E-04 6.8E-02 2.28E-05 4.98E-04 4.07E-02 -2.78E-01
PM = Potential incidence of disease due to PM emissions; IR = Potential Human exposure efficiency relative to U235; ETP-fw = Potential comparative
Toxic Unit for ecosystems; HTP-c = Potential comparative Toxic Unit for humans (cancerogenic); HTP-nc = Potential comparative Toxic Unit for humans
(not cancerogenic); SQP = Potential soil quality index
Disclaimer 1 – for the indicator 'Potential Human exposure efficiency relative to U235'. This impact category deals mainly with the
eventual impact of low-dose ionizing radiation on human health of the nuclear fuel cycle. It does not consider effects due to possible
nuclear accidents, occupational exposure or radioactive waste disposal in underground facilities. Potential ionizing radiation from the
soil, radon and from some construction materials is also not measured by this indicator.
Disclaimer 2 – for the indicators 'abiotic depletion potential for non-fossil resources', 'abiotic depletion potential for fossil resources',
'water (user) deprivation potential, deprivation-weighted water consumption', 'potential comparative toxic unit for ecosystems', 'potential
comparative toxic unit for humans – cancerogenic', 'Potential comparative toxic unit for humans - not cancerogenic', 'potential soil
quality index'. The results of this environmental impact indicator shall be used with care as the uncertainties on these results are high
as there is limited experience with the indicator. This EPD was created using a software tool.
References
Standards
LCA for Expert
EN 15804 Life cycle assessment software (version 10), by
SpheraSolutions GmbH, Leinfelden-Echterdingen,
EN 15804:2012+A1 2013, Sustainability of construction works 2022https://sphera.com/life-cycle-assessment-lca-software/
— Environmental Product Declarations — Core rules for the
product category of construction products. Managed LCA Content
Life cycle assessment database, by Sphera Solutions
EN 15804 GmbH,Leinfelden-Echterdingen, 2022https://sphera.com/life-
cycle-assessment-lca-database/
EN 15804:2012+A2:2019+AC:2021, Sustainability of
construction works — Environmental Product Declarations — PCR Part A
Core rules for the product category of construction products. PCR - Part A: Calculation rules for the Life Cycle
Assessmentand Requirements on the Background Report,
ISO 14025 version 1.3,Institut Bauen und Umwelt e.V., 08-2021.
EN ISO 14025:2011, Environmental labels and declarations — PCR Part B
Type III environmental declarations — Principles and PCR – Part B:Requirements on the EPD for Concrete
procedures. admixtures, Institut Bauen und Umwelt e.V., 04-2023.
Further References SN EN 934-2
Plasticizer for concrete
Title of the software/database
SN EN 934-2+A1,
Title of the software/database. Addition to the title, version.
Admixtures for concrete, mortar and grout – Part 2
Place: Publisher, Date of publication [Access on access date].
ISO 15686:1, -2, -7 and -8
IBU 2021
Buildings and constructed assets - Service life planning: Part 1,
General principles and framework
Institut Bauen und Umwelt e.V.: General Instructions for the
Buildings and constructed assets - Service life planning: Part 2,
EPD programme of Institut Bauen und Umwelt e.V., Version
Service life prediction procedures
2.0, Berlin: Institut Bauen und Umwelt e.V., 2021
Buildings and constructed assets - Service life planning: Part 7,
www.ibu-epd.com
Performance evaluation for feedback of service life data from
practice
LCA Calculator
Buildings and constructed assets - Service life planning: Part 8,
LCA Calculator software (version 6). Visualize, Improve
Reference service life and service-life estimation
andReport on Product Sustainability. https://sphera.com/your-
path[1]to-sustainability/
5 Environmental Product Declaration - Sika Schweiz AG - Sika® ViscoCrete®-4097
Publisher
Institut Bauen und Umwelt e.V. +49 (0)30 3087748- 0
Hegelplatz 1 info@ibu-epd.com
10117 Berlin www.ibu-epd.com
Germany
Programme holder
Institut Bauen und Umwelt e.V. +49 (0)30 3087748- 0
Hegelplatz 1 info@ibu-epd.com
10117 Berlin www.ibu-epd.com
Germany
Author of the Life Cycle Assessment
Sika Technology AG +41 (0)58 436 40 40
Tüffenwies 16 product.sustainability@ch.sika.com
8048 Zürich www.sika.com/sustainability
Switzerland
Owner of the Declaration
Sika Schweiz AG +41(0)58 436 40 40
Tüffenwies 16 kurz.christophe@ch.sika.com
8048 Zürich https://che.sika.com/
Switzerland
6 Environmental Product Declaration - Sika Schweiz AG - Sika® ViscoCrete®-4097
