ENVIRONMENTAL PRODUCT DECLARATION
as per ISO 14025 and EN 15804+A2
Owner of the Declaration danfloor a/s
Programme holder Institut Bauen und Umwelt e.V. (IBU)
Publisher Institut Bauen und Umwelt e.V. (IBU)
Declaration number EPD-DAN-20220311-CBA1-EN
Issue date 31.01.2023
Valid to 30.01.2028
Tufted wall-to-wall carpet
With a maximum total pile weight of 1215 g/m2, 95%
regenerated PA6, SBR based textile backing
danfloor a/s
www.ibu-epd.com | https://epd-online.com
Umwelt Produktdeklaration Name des Herstellers – Name des Produkts
General Information
danfloor a/s Tufted wall-to-wall carpet
With a maximum total pile weight of
1215 g/m2, 95 % regenerated PA6,
SBR based textile backing
Programme holder Owner of the declaration
IBU – Institut Bauen und Umwelt e.V. danfloor a/s
Hegelplatz 1 Østerbro 9
10117 Berlin 6933 Kibæk
Germany Denmark
www.danfloor.com
Declaration number Declared product / declared unit
EPD-DAN-20220311-CBA1-EN 1 m² tufted wall-to-wall carpet, PA 6 pile material with a
SBR based textile backing
This declaration is based on the product Scope:
category rules: The manufacturer declaration applies to tufted wall-to-
Floor coverings, 02/2018 wall carpet with a SBR based textile backing, a pile
(PCR checked and approved by the SVR) material of 95 % recycled PA 6 with a maximum total
pile weight of 1215 g/m2. The products are produced in
Kibæk, Denmark and coated in Bording, Denmark.
Issue date
LCA results for products with a maximum total pile
31.01.2023
weight of 1120 g/m2 can be taken from the
corresponding tables of the annexe. Specific data for
Valid to every product within the declared group of products in
30.01.2028 relation to its total pile weight can be calculated by
using equation 1 given in the annexe (see annexe
chapter: 'General Information on the annexe'). The
declaration is only valid in conjunction with a valid
GUT-PRODIS license of the product.
The owner of the declaration shall be liable for the
underlying information and evidence; the IBU shall not
be liable with respect to manufacturer information, life
cycle assessment data and evidences.
The EPD was created according to the specifications
of EN 15804+A2. In the following, the standard will be
simplified as EN 15804.
Verification
The standard EN 15804 serves as the core PCR
Independent verification of the declaration and data
according to ISO 14025:2011
Dipl. Ing. Hans Peters internally x externally
(chairman of Institut Bauen und Umwelt e.V.)
Dr. Alexander Röder Angela Schindler
(Managing Director Institut Bauen und Umwelt e.V.)) (Independent verifier)
Product
Product description/Product definition Regulation (EU) No. 305/2011 Construction Product
The declaration applies to tufted wall-to-wall carpet Regulation (CPR) applies. The product needs a
having a surface pile of 95 % recycled solution-dyed Declaration of Performance (DoP) taking into
polyamide 6 with a maximum total pile weight of 1215 consideration EN 14041:2018-05, Resilient, textile and
g/m2. The backing of the carpet consists of a SBR laminate floor coverings - Essential characteristics, and
based textile backing. The total recycled content of the the CE-marking. The DoP of the product can be found
carpet is 42 %. on the manufacturer's technical information section.
For the application and use of the product the
For the placing on the market of the specific product in respective national provisions apply.
the European Union/European Free Trade Association
(EU/EFTA) (with the exception of Switzerland)
2 Environmental Product Declaration danfloor – Tufted wall-to-wall carpet, 95% recycled polyamide 6 with a maximum total
pile weight of 1215 g/m2 and a textile backing
Application Additives 1.1 %
The use class of the specific product as defined in
EN 1307 can be found in the Product Information The specific product coverd by the EPD contains
System (PRODIS) using the PRODIS registration substances listed in the ECHA candidate list
number of the product. (08.07.2021) or other carcinogenic, mutagenic or
reprotoxic (CMR) substances in categories 1A or 1B
Technical Data which are not on the candidate list exceeding 0.1
percentage by mass: no
The products are registered in the GUT-PRODIS
Constructional data according to EN 1307 Information System. The PRODIS system ensures
Name Value Unit compliance with limitations of various chemicals and
Product Form Wall-to-wall carpet on rolls - Volatile Organic Compounds (VOC)-emissions and a
Type of manufacture Tufted carpet - ban on the use of all substances that are listed as
Yarn type Polyamide 6 - 'Substances of Very High Concern' (SVHC) under
Total carpet weight 3047 g/m2 REACH.
Secondary backing SBR based textile backing -
Reference service life
The service life of textile floor coverings strongly
Performance data of the product in accordance with depends on the correct installation taking into account
the declaration of performance with respect to its the declared use classification and the adherence to
essential characteristics according to EN 14041: 2018- cleaning and maintenance instructions.
05, Resilient, textile and laminate floor coverings - A calculation of the reference service life according to
Essential characteristics. ISO 15686 is not possible.
Additional product properties in accordance with EN Alternatively, a reference service life of 10 years can
1307 can be found on the Product Information System be assumed, during which the functional and visual
PRODIS using the PRODIS registration number of the quality is guaranteed (BNB, Nutzungsdauer von
product (www.pro-dis.info) or on the manufacturer's Bauteilen). The technical service life can be
technical information section. significantly longer.
Base materials/Ancillary materials
Name Value Unit
Polyamide 6 39.9 %
Polypropylene 2.6 %
Polyester 4.3 %
Polymer dispersion 12.9 %
Limestone 20.7 %
ATH 18.5 %
LCA: Calculation rules
Declared Unit Energy supply and production of the basic material,
processing of secondary material, auxiliary material,
transport of the material to the manufacturing site,
Name Value Unit emissions, waste water treatment, packaging material
Declared unit 1 m2 and waste processing up to the landfill disposal of
Grammage 3.047 kg/m2 residual waste (except radioactive waste). Benefits for
The declared unit refers to 1 m2 produced textile floor generated electricity and steam due to the incineration
covering. The Output of module A5 'Assembly' is 1 m2 of production waste are aggregated.
installed textile floor covering. Biogenic carbon that is stored in renewable material
The layer thickness of the specific product covered by (packaging paper) is taken into account as well as the
the EPD can be found on the Product Information associated carbon dioxide uptake from the air from
System PRODIS using the PRODIS registration which this biogenic carbon comes.
number of the product (www.pro-dis.info) or on the
manufacturer's technical information section. A4 Transport:
Transport of the packed textile floor covering
from factory gate to the place of installation.
System boundary A5 Installation:
Installation of the textile floor covering, processing of
Type of EPD: Cradle-to-grave installation waste and packaging waste up to the
System boundaries of modules A, B, C, D: landfill disposal of residual waste (except radioactive
Modules C3, C4 and D are indicated separately for waste), the production of the amount of carpet that
three end-of-life scenarios: occurs as installation waste including its transport to
1 - landfill disposal the place of installation.
2 - municipal waste incineration Generated electricity and steam due to the incineration
3 - recovery in a cement plant of waste are listed in the result table as exported
energy.
A1-A3 Production:
3 Environmental Product Declaration danfloor – Tufted wall-to-wall carpet, 95% recycled polyamide 6 with a maximum total
pile weight of 1215 g/m2 and a textile backing
Biogenic carbon that is stored in renewable materials C3 Waste processing:
in packaging paper is released as carbon dioxide C3-1: Landfill disposal needs no waste processing.
emissions into the air at the end of life in module A5. C3-2: Impact from waste incineration (plant with
Preparation of the floor and auxiliary materials R1>0.6), generated electricity and steam are listed in
(adhesives, fixing agents, PET connectors) are beyond the result table as exported energy.
the system boundaries and not taken into account. C3-3: Collection of the carpet waste for recovery in the
cement industry, waste processing (granulating),
B1 Use: transport to the cement plant, emissions from the
Indoor emissions during the use stage. After the first incineration.
year, no product-related Volatile Organic Compound
(VOC) emissions are relevant due to known VOC C4 Disposal
decay curves of the product. C4-1: Impact from landfill disposal,
C4-2: The carpet waste leaves the system in
B2 Maintenance: module C3-2,
Cleaning of the textile floor covering for a period of 1 C4-3: The pre-processed carpet waste leaves the
year: system in module C3-3.
Vacuum cleaning – electricity supply
Wet cleaning – electricity, water consumption, D Recycling potential:
production of the cleaning agent, waste water Calculated benefits result from materials exclusive
treatment. secondary materials (net materials).
The declared values in this module have to be D-A5: Benefits for generated energy due
multiplied by the assumed service life of the floor to incineration of packaging and installation waste
covering in the building in question. (incineration plant with R1 > 0.6),
D-1: Benefits for generated energy due to landfill
B3 - B5: disposal of carpet waste at the end-of-life,
The modules are not relevant within the assumed D-2: Benefits for generated energy due to incineration
reference service life of 10 years. of carpet waste at the end-of-life (incineration plant
with R1 > 0.6),
B6 - B7: D-3: Benefits for saved fossil energy and saved
No energy and water input are required for the inorganic material due to recovery of the carpet in a
operation of the carpet in the use stage. The modules cement plant.
do not cause any environmental impact.
Comparability
C1 De-construction: Basically, a comparison or an evaluation of EPD data
The floor covering is de-constructed manually and no is only possible if all the data sets to be compared
additional environmental impact is caused. were created according to EN 15804 and the building
context, respectively the product-specific
C2 Transport: characteristics of performance, are taken into account.
Transport of the carpet waste to a landfill, to the
municipal waste incineration plant (MWI) or to the Background data are taken from the GaBi database,
waste collection facility for recycling. 2021-2. Remaining data gaps are covered by the
ecoinvent 3.7 database, 2020.
LCA: Scenarios and additional technical information
Characteristic product properties incineration plant. Cardboard packaging waste is going
Information on biogenic carbon to be recycled.
Preparation of the floor and auxiliaries (adhesives,
fixing agents, PET connectors etc.) are not taken into
Name Value Unit account.
Biogenic carbon content in
accompanying packaging at 0.022 kg C Maintenance (B2)
factory gate The values for cleaning refer to 1 m2 floor covering per
1 kg biogenic Carbon is equivalent to 44/12 kg of CO year.
2
Depending on the application based on ISO 10874, the
technical service life recommended by the
manufacturer and the anticipated strain on the floor by
Transport to the construction site (A4) customers, the case-specific useful life can be
Name Value Unit established. Based on this useful life the effects of
Litres of fuel (truck, EURO 0-6 module B2 need to be calculated in order to obtain the
0.0071 l/100km
mix) overall environmental impacts.
Transport distance 700 km Name Value Unit
Capacity utilisation (including Maintenance cycle (vacuum Number
55 % 208
empty runs) cleaning) /year
Number
Maintenance cycle (wet cleaning) 1,5
Installation in the building (A5) /year
Name Value Unit Water consumption (wet cleaning) 0.004 m3
Material loss 0.274 kg Cleaning agent (wet cleaning) 0.09 kg
Polyethylene packaging waste and installation waste Electricity consumption 0.314 kWh
are considered to be incinerated in a municipal waste
4 Environmental Product Declaration danfloor – Tufted wall-to-wall carpet, 95% recycled polyamide 6 with a maximum total
pile weight of 1215 g/m2 and a textile backing
For further information on cleaning and maintenance
see www.danfloor.com
Service life
Name Value Unit
Life Span (according to
10 a
BBSR)
Declared product Corresponds to the
properties (at the gate) specifications of EN -
and finishes 1307
An assumed quality of
work, when installed in Conforms to the
accordance with the manufacturer's -
manufacturer’s instructions
instructions
Usage conditions, e.g. Use in areas defined by
frequency of use, the use class according -
mechanical exposure to EN 1307
Maintenance e.g. required
According to the
frequency, type and
manufacturers -
quality and replacement of
instructions
components
End of Life (C1-C4)
Three different end-of-life scenarios are declared and
the results are indicated separately in module C.
Each scenario is calculated as a 100% scenario.
Scenario 1: 100 % landfill disposal
Scenario 2: 100 % municipal waste incineration (MWI)
with R1>0.6
Scenario 3: 100 % recovery in the cement industry
If combinations of these scenarios have to be
calculated this should be done according to the
following scheme:
EOL-impact = x % impact (Scenario 1)
+ y % impact (Scenario 2)
+ z % impact (Scenario 3)
with x % + y % + z % = 100 %
Name Value Unit
Collected as mixed construction
3.047 kg
waste (scenarios 1 and 2)
Collected separately (scenario 3) 3.047 kg
Landfilling (scenario 1) 3.047 kg
Energy recovery (scenario 2) 3.047 kg
Energy recovery (scenario 3) 1.853 kg
Recycling (scenario 3) 1.194 kg
Reuse, recovery and/or recycling potentials (D),
relevant scenario information
Recovery or recycling potentials due to the three end-
of-life scenarios (module C) are indicated separately.
Recycling in the cement industry (scenario 3)
The organic material of the carpet is used as an
alternative fuel in a cement kiln. It mainly substitutes
for lignite (68.8 %), hard coal (23.6 %) and petrol coke
(7.6 %). The inorganic material is substantially
integrated into the cement clinker and substitutes for
original material input. VDZ e.V.
5 Environmental Product Declaration danfloor – Tufted wall-to-wall carpet, 95% recycled polyamide 6 with a maximum total
pile weight of 1215 g/m2 and a textile backing
LCA: Results
The LCA results refer to all declared products with a maximum total pile weight of 1215 g/m2. LCA results for
products with a maximum total pile weight of 1120 g/m2 can be taken from the corresponding tables of the
annexe. Results for specific products with any other total pile weight can be calculated by using equation 1 given
in the annexe (see annexe chapter: 'General Information on the annexe'). The declared result figures in module
B2 have to be multiplied by the assumed service life (in years) of the floor covering in the building under
consideration. Information on non-relevant modules: Modules B3 - B7 are not relevant during the service life of
the carpet. Modules C1, C3/1, C4/2 and C4/3 cause no additional impact (see chapter "LCA: Calculation rules" in
this document). All these modules are declared and marked as 'modules not relevant/declared'. Module C2
represents the transport for scenarios 1, 2 and 3. Column D represents module D/A5.
DESCRIPTION OF THE SYSTEM BOUNDARY (X = INCLUDED IN LCA; ND = MODULE OR INDICATOR NOT
DECLARED; MNR = MODULE NOT RELEVANT)
BENEFITS AND
CONSTRUCTI LOADS
PRODUCT STAGE ON PROCESS USE STAGE END OF LIFE STAGE BEYOND THE
STAGE SYSTEM
BOUNDARIES
6 Environmental Product Declaration danfloor – Tufted wall-to-wall carpet, 95% recycled polyamide 6 with a maximum total
pile weight of 1215 g/m2 and a textile backing
lairetam
waR
ylppus tropsnarT
gnirutcafunaM
eht
morf
tropsnarT
etis
eht
ot
etag
ylbmessA esU
ecnanetniaM
riapeR
tnemecalpeR tnemhsibrufeR
ygrene
lanoitarepO esu
retaw
lanoitarepO esu
noitcurtsnoc-eD
noitilomed tropsnarT
gnissecorp
etsaW
lasopsiD -esueR -yrevoceR -gnilcyceR laitnetop
A1 A2 A3 A4 A5 B1 B2 B3 B4 B5 B6 B7 C1 C2 C3 C4 D
X X X X X X X MNR MNR MNR ND ND X X X X X
RESULTS OF THE LCA - ENVIRONMENTAL IMPACT according to EN 15804+A2: 1 m² floor covering
Core Indicator Unit A1-A3 A4 A5 B1 B2 C1 C2 C3/2 C3/3 C4/1 D D/1 D/2 D/3
GWP-total [kg CO2-Eq.] 5.27E+01.85E-11.07E+00.00E+04.16E-10.00E+01.03E-24.20E+04.24E+02.16E-1-3.95E-20.00E+0-2.62E-1-2.63E-1
GWP-fossil [kg CO2-Eq.] 5.31E+01.81E-1 9.07E-10.00E+02.15E-10.00E+01.02E-24.20E+04.24E+02.16E-1-3.93E-20.00E+0-2.61E-1-2.63E-1
GWP-biogenic [kg CO2-Eq.] -5.16E-22.35E-3 1.72E-10.00E+04.16E-30.00E+01.31E-4 5.67E-4 1.04E-30.00E+0-1.96E-40.00E+0-1.27E-3-5.24E-4
GWP-luluc [kg CO2-Eq.] 8.96E-3 1.03E-3 9.15E-40.00E+01.96E-10.00E+05.75E-5 1.29E-4 2.76E-4 1.05E-4-4.19E-60.00E+0-2.71E-5-1.52E-4
1.10E- 6.18E- 4.03E- 6.33E- 2.90E- -2.55E- -1.64E- -1.80E-
ODP [kg CFC11-Eq.] 1.43E-8 1.28E-90.00E+03.42E-80.00E+0 0.00E+0
14 16 13 13 13 13 12 13
AP [mol H+-Eq.] 2.02E-2 1.10E-3 2.42E-30.00E+08.32E-40.00E+06.14E-5 5.48E-3 5.67E-3 6.40E-4-5.05E-50.00E+0-3.30E-4-1.29E-3
EP-freshwater [kg P-Eq.] 6.43E-5 5.49E-7 5.88E-60.00E+05.19E-60.00E+03.08E-8 5.02E-7 6.25E-7 4.03E-5-5.20E-80.00E+0-3.35E-7-3.29E-7
EP-marine [kg N-Eq.] 7.14E-3 5.38E-4 9.41E-40.00E+01.97E-40.00E+03.01E-5 2.74E-3 2.83E-3 1.42E-4-1.38E-50.00E+0-9.09E-5-3.56E-4
EP-terrestrial [mol N-Eq.] 6.61E-2 5.96E-3 9.27E-30.00E+02.83E-30.00E+03.34E-4 3.05E-2 3.14E-2 1.55E-3-1.48E-40.00E+0-9.76E-4-3.90E-3
POCP [kg NMVOC-Eq.]1.69E-2 1.02E-3 2.25E-3 4.18E-4 9.83E-40.00E+05.70E-5 7.01E-3 7.18E-3 4.56E-4-3.88E-50.00E+0-2.55E-4-1.03E-3
8.62E-
ADPE [kg Sb-Eq.] 1.44E-6 1.54E-8 1.33E-70.00E+02.30E-70.00E+0 1.94E-8 2.58E-8 1.50E-8-5.77E-90.00E+0-3.75E-8-2.79E-8
10
- -
ADPF [MJ] 9.33E+12.46E+08.85E+00.00E+05.90E+00.00E+01.38E-12.42E+03.05E+03.06E+0-6.66E-10.00E+0
4.41E+01.59E+1
[m³ world-Eq
WDP 6.99E+01.65E-3 6.81E-10.00E+09.99E-20.00E+09.22E-5 5.47E-1 5.51E-1-2.29E-3-3.98E-30.00E+0-2.56E-2-3.26E-2
deprived]
GWP = Global warming potential; ODP = Depletion potential of the stratospheric ozone layer; AP = Acidification potential of land and water; EP =
Caption Eutrophication potential; POCP = Formation potential of tropospheric ozone photochemical oxidants; ADPE = Abiotic depletion potential for non-
fossil resources; ADPF = Abiotic depletion potential for fossil resources; WDP = Water (user) deprivation potential
RESULTS OF THE LCA - INDICATORS TO DESCRIBE RESOURCE USE according to EN 15804+A2: 1 m²
floor covering
Indicator Unit A1-A3 A4 A5 B1 B2 C1 C2 C3/2 C3/3 C4/1 D D/1 D/2 D/3
PERE [MJ] 6.56E+1 1.40E-1 6.05E+0 0.00E+0 3.69E+0 0.00E+0 7.84E-3 3.74E-1 5.51E-1 2.52E-1 -1.77E-1 0.00E+0 -1.14E+0-4.82E-1
PERM [MJ] 9.70E-2 0.00E+0 -9.70E-2 0.00E+0 0.00E+0 0.00E+0 0.00E+0 0.00E+0 0.00E+0 0.00E+0 0.00E+0 0.00E+0 0.00E+0 0.00E+0
PERT [MJ] 6.57E+1 1.40E-1 5.96E+0 0.00E+0 3.69E+0 0.00E+0 7.84E-3 3.74E-1 5.51E-1 2.52E-1 -1.77E-1 0.00E+0 -1.14E+0-4.82E-1
PENRE [MJ] 7.76E+1 2.47E+0 9.32E+0 0.00E+0 5.90E+0 0.00E+0 1.38E-1 1.78E+1 1.84E+1 3.07E+0 -6.66E-1 0.00E+0 -4.42E+0-1.59E+1
PENRM [MJ] 1.58E+1 0.00E+0 -4.60E-1 0.00E+0 0.00E+0 0.00E+0 0.00E+0 -1.54E+1-1.54E+1 0.00E+0 0.00E+0 0.00E+0 0.00E+0 0.00E+0
PENRT [MJ] 9.34E+1 2.47E+0 8.86E+0 0.00E+0 5.90E+0 0.00E+0 1.38E-1 2.43E+0 3.05E+0 3.07E+0 -6.66E-1 0.00E+0 -4.42E+0-1.59E+1
SM [kg] 1.46E+0 0.00E+0 1.31E-1 0.00E+0 0.00E+0 0.00E+0 0.00E+0 0.00E+0 0.00E+0 0.00E+0 0.00E+0 0.00E+0 0.00E+0 7.20E-1
RSF [MJ] 0.00E+0 0.00E+0 0.00E+0 0.00E+0 0.00E+0 0.00E+0 0.00E+0 0.00E+0 0.00E+0 0.00E+0 0.00E+0 0.00E+0 0.00E+0 0.00E+0
NRSF [MJ] 0.00E+0 0.00E+0 0.00E+0 0.00E+0 0.00E+0 0.00E+0 0.00E+0 0.00E+0 0.00E+0 0.00E+0 0.00E+0 0.00E+0 0.00E+0 0.00E+0
FW [m³] 1.67E-1 1.58E-4 1.63E-2 0.00E+0 3.34E-3 0.00E+0 8.85E-6 1.29E-2 1.31E-2 3.59E-5 -1.69E-4 0.00E+0 -1.09E-3 -1.84E-3
PERE = Use of renewable primary energy excluding renewable primary energy resources used as raw materials; PERM = Use of
renewable primary energy resources used as raw materials; PERT = Total use of renewable primary energy resources; PENRE = Use of
non-renewable primary energy excluding non-renewable primary energy resources used as raw materials; PENRM = Use of non-
Caption
renewable primary energy resources used as raw materials; PENRT = Total use of non-renewable primary energy resources; SM = Use
of secondary material; RSF = Use of renewable secondary fuels; NRSF = Use of non-renewable secondary fuels; FW = Use of net fresh
water
RESULTS OF THE LCA – WASTE CATEGORIES AND OUTPUT FLOWS according to EN 15804+A2:
1 m² floor covering
Indicator Unit A1-A3 A4 A5 B1 B2 C1 C2 C3/2 C3/3 C4/1 D D/1 D/2 D/3
HWD [kg] 3.57E-3 1.18E-11 3.21E-4 0.00E+0 4.19E-5 0.00E+0 6.62E-133.82E-104.08E-104.73E-10-9.13E-110.00E+0-6.11E-10-3.78E-10
NHWD [kg] 7.75E-1 3.53E-4 1.26E-1 0.00E+0 7.30E-3 0.00E+0 1.98E-5 6.27E-1 6.28E-1 3.03E+0 -3.31E-4 0.00E+0 -2.16E-3 -2.68E-1
RWD [kg] 2.01E-3 3.04E-6 1.89E-4 0.00E+0 3.76E-4 0.00E+0 1.70E-7 7.98E-5 1.25E-4 3.77E-5 -5.06E-5 0.00E+0 -3.25E-4 -1.11E-4
CRU [kg] 0.00E+0 0.00E+0 0.00E+0 0.00E+0 0.00E+0 0.00E+0 0.00E+0 0.00E+0 0.00E+0 0.00E+0 0.00E+0 0.00E+0 0.00E+0 0.00E+0
MFR [kg] 3.16E-2 0.00E+0 5.27E-2 0.00E+0 0.00E+0 0.00E+0 0.00E+0 0.00E+0 7.20E-1 0.00E+0 0.00E+0 0.00E+0 0.00E+0 0.00E+0
MER [kg] 0.00E+0 0.00E+0 0.00E+0 0.00E+0 0.00E+0 0.00E+0 0.00E+0 0.00E+0 0.00E+0 0.00E+0 0.00E+0 0.00E+0 0.00E+0 0.00E+0
EEE [MJ] 0.00E+0 0.00E+0 6.91E-1 0.00E+0 0.00E+0 0.00E+0 0.00E+0 6.88E+0 0.00E+0 0.00E+0 0.00E+0 0.00E+0 0.00E+0 0.00E+0
EET [MJ] 0.00E+0 0.00E+0 1.26E+0 0.00E+0 0.00E+0 0.00E+0 0.00E+0 1.26E+1 5.35E+1 0.00E+0 0.00E+0 0.00E+0 0.00E+0 0.00E+0
HWD = Hazardous waste disposed; NHWD = Non-hazardous waste disposed; RWD = Radioactive waste disposed; CRU = Components
Caption for re-use; MFR = Materials for recycling; MER = Materials for energy recovery; EEE = Exported electrical energy; EET = Exported
thermal energy
RESULTS OF THE LCA – additional impact categories according to EN 15804+A2-optional:
1 m² floor covering
Indicator Unit A1-A3 A4 A5 B1 B2 C1 C2 C3/2 C3/3 C4/1 D D/1 D/2 D/3
[Disease -4.18E-
PM 1.52E-7 6.33E-9 1.60E-8 0.00E+0 6.84E-8 0.00E+03.55E-10 1.92E-8 2.04E-8 6.15E-9 0.00E+0 0.00E+0 -2.35E-8
Incidence] 10
[kBq U235-
IRP 3.26E-1 4.45E-4 3.05E-2 0.00E+0 6.78E-2 0.00E+0 2.49E-5 1.21E-2 1.99E-2 5.56E-3 -8.57E-3 0.00E+0 0.00E+0 -1.54E-2
Eq.]
ETP-fw [CTUe] 4.82E+1 1.71E+0 4.60E+0 3.60E-3 2.69E+0 0.00E+0 9.57E-2 1.04E+0 1.40E+0 3.00E+0 -1.41E-1 0.00E+0 0.00E+0-3.54E+0
-6.66E- -8.05E-
HTP-c [CTUh] 2.82E-9 3.45E-112.62E-100.00E+06.21E-100.00E+01.93E-125.53E-116.37E-111.35E-10 0.00E+0 0.00E+0
12 11
-2.56E-
HTP-nc [CTUh] 1.17E-7 2.05E-9 1.10E-8 2.60E-11 9.46E-9 0.00E+01.15E-10 3.48E-9 3.90E-9 1.13E-8 0.00E+0 0.00E+0 -5.85E-9
10
SQP [-] ND ND ND ND ND ND ND ND ND ND ND ND ND ND
PM = Potential incidence of disease due to PM emissions; IR = Potential Human exposure efficiency relative to U235; ETP-fw = Potential
Caption comparative Toxic Unit for ecosystems; HTP-c = Potential comparative Toxic Unit for humans (cancerogenic); HTP-nc = Potential
comparative Toxic Unit for humans (not cancerogenic); SQP = Potential soil quality index
No substantiated values can be given for the SQP indicator with the existing database.
The result figures given in module B2 refer to a period of 1 year because a reference service life is not declared.
They have to be multiplied by the assumed service life (in years) of the floor covering in the building under
consideration.
Disclaimer 1 – for the indicator “Potential Human exposure efficiency relative to U235”.
This impact category deals mainly with the eventual impact of low dose ionizing radiation on human health of the
nuclear fuel cycle. It does not consider effects due to possible nuclear accidents, occupational exposure or
radioactive waste disposal in underground facilities. Potential ionizing radiation from the soil, from radon and from
some construction materials is also not measured by this indicator.
Disclaimer 2 – for the indicators “abiotic depletion potential for non-fossil resources”, “abiotic depletion potential
for fossil resources”, “water (user) deprivation potential, deprivation-weighted water consumption”, “potential
comparative toxic unit for ecosystems”, “potential comparative toxic unit for humans – cancerogenic”, “Potential
comparative toxic unit for humans - not cancerogenic”, “potential soil quality index”.
The results of this environmental impact indicator shall be used with care as the uncertainties on these results are
high or as there is limited experience with the indicator.
References
EN 1307 floor coverings – Environmental product declarations –
DIN EN 1307: 2014+A1:2016+A2:2018-05: Textile Product category rules
floor coverings - Classification
ISO 10874
EN 13501-1 DIN EN ISO 10874: 2012+A1:2021-04: Resilient,
DIN EN 13501-1:2019-05: Fire classification of textile and laminate floor coverings - Classification
construction products and building elements - Part 1:
Classification using data from reaction to fire tests ISO 14025
DIN EN /ISO 14025:2011-10/, Environmental labels
EN 14041 and declarations — Type III environmental
DIN EN 14041: 2018-05 and DIN EN 14041: 2008-05: declarations — Principles and procedures
Resilient, textile and laminate floor coverings -
Essential characteristics
ISO 14040
EN 15804 DIN EN ISO 14040:2006+A1:2020 Environmental
DIN EN 15804:2012+A2:2019+AC:2021, Sustainability management - Life cycle assessment - Principles and
of construction works — Environmental Product framework
Declarations — Core rules for the product category of
construction products ISO 14044
DIN EN ISO 14044:2006+A1:2018+A2:2020
EN 16810 Environmental management - Life cycle assessment -
DIN EN 16810: 2017-08: Resilient, textile and laminate Requirements and guidelines
7 Environmental Product Declaration danfloor – Tufted wall-to-wall carpet, 95% recycled polyamide 6 with a maximum total
pile weight of 1215 g/m2 and a textile backing
ISO 15686 GaBi database
ISO 15686: Buildings and constructed assets - GaBi Software-System and Database for Life Cycle
Service life planning Engineering, thinkstep AG, Leinfelden-Echterdingen,
ISO 15686-1: 2011-05: Part 1: General principles and 2022-1
framework
ISO 15686-2: 2012-05: Part 2: Service life prediction PCR Part A
procedures Product Category Rules for Building-Related Products
ISO 15686-7: 2017-04: Part 7: Performance and Services Part A: Calculation Rules for the Life
evaluation for feedback of service life data Cycle Assessment and Requirements on the Project
from practice Report according to EN 15804+A2:2019, V1.1, Berlin:
ISO 15686-8: 2008-06: Part 8: Reference service life Institut Bauen und Umwelt e.V. (IBU), January 2021
and service-life estimation
PCR Part B
Regulation (EU) No. 305/2011 Product Category Rules for Building-Related Products
Regulation No. 305/2011 Construction Products and Services
Regulation (CPR) of the European Council and of the Part B: Requirements on the EPD for floor coverings,
European Parliament, April 2011 V1.2, Berlin: Institut Bauen und Umwelt e.V. (IBU),
February 2018
General Instructions for the IBU-EPD Program
General Instructions for the EPD-Program of the PRODIS
Institut Bauen und Umwelt e.V., The Preparation of Product Information System (PRODIS) of the
Environmental Product Declarations - EPDs, version European Carpet Industry, Gemeinschaft
2.0, Institut Bauen und Umwelt e.V., Berlin, January umweltfreundlicher Teppichboden e.V (GUT) and
2021, www.ibu-epd.de European Carpet and Rug Association
(ECRA), http://www.pro-dis.info
BNB, Nutzungsdauer von Bauteilen
Bewertungssystem Nachhaltiges Bauen (BNB), REACH
Nutzungsdauer von Bauteilen, Bundesministerium des Regulation (EC) No 1907/2006 of the European
Inneren, für Bau und Heimat, 24.02.2017 Parliament and of the Council of 18 December 2006
concerning the Registration, Evaluation, Authorisation
ECHA candidate list and Restriction of Chemicals (REACH), June 2017,
Candidate List of substances of very high concern last update: 08.07.2021
(SVHCs) for authorisation, 08.07.2021, European
Chemicals Agency (ECHA), Helsinki, Finland VDZ e.V.
Association of German Cement Works, Ed. Environ-
mental Data of the German Cement Industry 2020
ecoinvent
ecoinvent, Zurich, Switzerland, database version 3.7,
published September 2020
8 Environmental Product Declaration danfloor – Tufted wall-to-wall carpet, 95% recycled polyamide 6 with a maximum total
pile weight of 1215 g/m2 and a textile backing
Publisher
Institut Bauen und Umwelt e.V. Tel +49 (0)30 3087748- 0
Hegelplatz 1 Fax +49 (0)30 3087748- 29
10117 Berlin Mail info@ibu-epd.com
Germany Web www.ibu-epd.com
Programme holder
Institut Bauen und Umwelt e.V. Tel +49 (0)30 - 3087748- 0
Hegelplatz 1 Fax +49 (0)30 – 3087748 - 29
10117 Berlin Mail info@ibu-epd.com
Germany Web www.ibu-epd.com
Author of the Life Cycle
Assessment Tel +49 (0)241 96843 410
Gemeinschaft umweltfreundlicher Fax +49 (0)241 96843 400
Teppichboden (GUT) e.V. Mail mail@gut-ev.de
Schönebergstraße 2 Web www.gut-ev.org
52068 Aachen
Germany
Owner of the Declaration
danfloor a/s Tel +4596991900
Østerbro 9 Fax +4596991999
6933 Kibæk Mail sales@danfloor.com
Denmark Web www.danfloor.com
