ENVIRONMENTAL PRODUCT DECLARATION
as per ISO 14025 and EN 15804+A1
Owner of the Declaration Balsan
Programme holder Institut Bauen und Umwelt e.V. (IBU)
Publisher Institut Bauen und Umwelt e.V. (IBU)
Declaration number EPD-BAL-20210259-CBA1-EN
Issue date 27.10.2021
Valid to 26.10.2026
TAKE A WALK
tufted carpet tiles made of recycled pile material
BALSAN
www.ibu-epd.com | https://epd-online.com
Umwelt Produktdeklaration Name des Herstellers – Name des Produkts
General Information
Balsan TAKE A WALK - tufted carpet tiles
made of recycled pile material
Programme holder Owner of the declaration
IBU – Institut Bauen und Umwelt e.V. Balsan
Panoramastr. 1 Corbilly - D14
10178 Berlin 36330 Arthon
Germany France
Declaration number Declared product / declared unit
EPD-BAL-20210259-CBA1-EN 1 m² tufted carpet tiles TAKE A WALK.
This declaration is based on the product Scope:
category rules: The manufacturer declaration applies to the tufted
Floor coverings, 02/2018 carpet tiles TAKE A WALK with the GUT-PRODIS
(PCR checked and approved by the SVR) license number A7BE310F.
The products are produced in the Balsan
Issue date manufacturing sites Arthon (tufting, dyeing and
precoating) and Neuvy-Saint-Sépulchre (back coating),
27.10.2021
France.
The declaration is only valid in conjunction with a valid
Valid to
GUT-PRODIS license of the product.
26.10.2026
The owner of the declaration shall be liable for the
underlying information and evidence; the IBU shall not
be liable with respect to manufacturer information, life
cycle assessment data and evidences.
The EPD was created according to the specifications
of EN 15804+A1. In the following, the standard will be
simplified as EN 15804.
Verification
The standard EN 15804 serves as the core PCR
Independent verification of the declaration and data
according to ISO 14025:2010
Dipl. Ing. Hans Peters internally x externally
(chairman of Institut Bauen und Umwelt e.V.)
Dr. Alexander Röder Angela Schindler
(Managing Director Institut Bauen und Umwelt e.V.)) (Independent verifier)
Product
Product description/Product definition For the application and use of the product the
TAKE A WALK - tufted carpet tiles having a surface respective national provisions apply.
pile of polyamide 6 with 100% recycled content, a
polyester primary backing with recycled content and a Application
bitumen based heavy backing with a fibre glass According to the use class as defined in EN 1307 the
reinforcement and a polyester covering fleece. products can be used in all professional areas which
The recycled content amounts to 18 %. require class 33 or less.
The tiles are coloured by a continuous dyeing method.
For the placing on the market of the product in the
European Union/European Free Trade Association
(EU/EFTA) (with the exception of Switzerland)
Regulation (EU) No. 305/2011 Construction Product
Technical Data
Regulation (CPR) applies. The product needs a
The performance data listed in the DoP apply.
Declaration of Performance (DoP) taking into
consideration EN 14041: 2018-05, Resilient, textile and
laminate floor coverings - Essential characteristics, and
the CE-marking. The DoP of the product can be found
on the manufacturer's technical information section.
2 Environmental Product Declaration Balsan – TAKE A WALK - tufted carpet tiles
Name Value Unit This product contains substances listed in the ECHA
Product Form Tiles 50 cm x 50 cm - candidate list (16.01.2020) or other carcinogenic,
Type of mutagenic or reprotoxic (CMR) substances in
Tufted tiles -
manufacture categories 1A or 1B which are not on the candidate list
Yarn type Polyamide 6, 100 % recycled - exceeding 0.1 percentage by mass: no
Coloration Continuous dyeing method The products are registered in the GUT-PRODIS
Primary backing Polyester, 90% recycled Information System. The PRODIS system ensures the
Secondary backing Bitumen based heavy backing - compliance with limitations of various chemicals and
Total pile weight 650 g/m² Volatile Organic Compound (VOC)-emissions and a
ban on the use of all substances that are listed as
Surface pile weight 370 g/m2
'Substances of Very High Concern' (SVHC) under
Total carpet weight 4030 g/m2
REACH.
Total thickness 6 mm
Reference service life
A calculation of the reference service life according to
Performance data of the product in accordance with
ISO 15686 is not possible.
the declaration of performance with respect to its
The service life of textile floor coverings strongly
essential characteristics according to EN 14041: 2018-
depends on the correct installation taking into account
05, Resilient, textile and laminate floor coverings -
the declared use classification and the adherence to
Essential characteristics. Additional product properties
cleaning and maintenance instructions.
in accordance with EN 1307 can be found on the
A minimum service life of 10 years can be
Product Information System PRODIS using the
assumed, technical service life can be considerably
PRODIS registration number of the product (www.pro-
longer.
dis.info) or on the manufacturer's technical information
section (www.balsan.com).
Base materials/Ancillary materials
Name Value Unit
Polyamide 6 16.1 %
Polyester 4.2 %
SBR-latex 4.2 %
Mineral filler 59.1 %
Bitumen 15.5 %
Glass fibre 0.9 %
LCA: Calculation rules
Declared Unit Biogenic carbon that is stored in renewable material
(packaging paper) is taken into account as well as the
associated carbon dioxide uptake from the air from
Name Value Unit which this biogenic carbon comes.
Declared unit 1 m2
Gross density 680 kg/m3 A4 Transport:
The declared unit refers to 1 m2 produced textile floor Transport of the packed textile floor covering
covering. The output of module A5 'Assembly' is 1 m2 from factory gate to the place of installation.
installed textile floor covering.
A5 Installation:
Installation of the textile floor covering, processing of
System boundary installation waste and packaging waste up to the
landfill disposal of residual waste (except radioactive
Type of EPD: Cradle-to-grave waste), the production of the amount of carpet that
occurs as installation waste including its transport to
System boundaries of modules A, B, C, D: the place of installation.
Modules C3, C4 and D are indicated separately for Generated electricity and steam due to the incineration
three end-of-life scenarios: of waste are listed in the result table as exported
1 - landfill disposal energy.
2 - municipal waste incineration Biogenic carbon that is stored in renewable materials
3 - recovery in a cement plant in packaging paper is released as carbon dioxide
emissions into the air at the end of life in module A5.
A1-A3 Production: Preparation of the floor and auxiliary materials
Energy supply and production of the basic material, (adhesives, fixing agents, PET connectors) are beyond
processing of secondary material, auxiliary material, the system boundaries and not taken into account.
transport of the material to the manufacturing site,
emissions, waste water treatment, packaging material B1 Use:
and waste processing up to the landfill disposal of Indoor emissions during the use stage. After the first
residual waste (except radioactive waste). Benefits for year, no product-related Volatile Organic Compound
generated electricity and steam due to the incineration (VOC) emissions are relevant due to known VOC
of production waste are aggregated. decay curves of the product.
3 Environmental Product Declaration Balsan – TAKE A WALK - tufted carpet tiles
B2 Maintenance:
Cleaning of the textile floor covering for a period of 1 C4 Disposal
year: C4-1: Impact from landfill disposal,
Vacuum cleaning – electricity supply C4-2: The carpet waste leaves the system in
Wet cleaning – electricity, water consumption, module C3-2,
production of the cleaning agent, waste water C4-3: The pre-processed carpet waste leaves the
treatment. system in module C3-3.
The declared values in this module have to be
multiplied by the assumed service life of the floor D Recycling potential:
covering in the building in question. Calculated benefits result from materials exclusive
secondary materials (net materials).
B3 - B7: D-A5: Benefits for generated energy due
The modules are not relevant and therefore not to incineration of packaging and installation waste
declared. (incineration plant with R1 > 0.6),
D-1: Benefits for generated energy due to landfill
C1 De-construction: disposal of carpet waste at the end-of-life,
The floor covering is de-constructed manually and no D-2: Benefits for generated energy due to incineration
additional environmental impact is caused. of carpet waste at the end-of-life (incineration plant
with R1 > 0.6),
C2 Transport: D-3: Benefits for saved fossil energy and saved
Transport of the carpet waste to a landfill, to the inorganic material due to recovery of the carpet in a
municipal waste incineration plant (MWI) or to the cement plant.
waste collection facility for recycling.
Comparability
C3 Waste processing: Basically, a comparison or an evaluation of EPD data
C3-1: Landfill disposal needs no waste processing. is only possible if all the data sets to be compared
C3-2: Impact from waste incineration (plant with were created according to EN 15804 and the building
R1>0.6), generated electricity and steam are listed in context, respectively the product-specific
the result table as exported energy. characteristics of performance, are taken into account.
C3-3: Collection of the carpet waste for recovery in the
cement industry, waste processing (granulating), Background data are taken from the GaBi database
transport to the cement plant, emissions from the 2021. Remaining data gaps are covered by the
incineration. The biogenic carbon that is stored in the ecoinvent 3.7 database
renewable materials of the floor covering is released
into the air as carbon dioxide emissions.
LCA: Scenarios and additional technical information
The following information refer to the declared modules Name Value Unit
and are the basis for calculations or can be used for Maintenance cycle (wet cleaning) 1.5 1/year
further calculations. Maintenance cycle (vacuum
208 1/year
cleaning)
Transport to the construction site (A4) Water consumption (wet cleaning) 0.004 m3
Name Value Unit Cleaning agent (wet cleaning) 0.09 kg
Litres of fuel (truck, EURO 0-6 mix) 0.0094 l/100km Electricity consumption 0.314 kWh
Transport distance 700 km Further information on cleaning and maintenance see
Capacity utilisation (including empty www.balsan.com
55 %
runs)
Gross density of products transported 680 kg/m3 End of Life (C1-C4)
Three different end-of-life scenarios are declared and
Installation in the building (A5) the results are indicated separately in module C.
Name Value Unit Each scenario is calculated as a 100% scenario.
Material loss 0.12 kg
Polyethylene packaging waste and installation waste Scenario 1: 100% landfill disposal
are considered to be incinerated in a municipal waste Scenario 2: 100% municipal waste incineration (MWI)
incineration plant. Cardboard is going to be recycled. with R1>0.6
Preparation of the floor and auxiliaries (adhesives, Scenario 3: 100% recycling in the cement industry
fixing agents, PET connectors etc.) are not taken into
account. If combinations of these scenarios have to be
calculated this should be done according to the
Maintenance (B2) following scheme:
The values for cleaning refer to 1 m2 floor covering EOL-impact = x% impact (Scenario 1)
used in commercial areas per year. Depending on the + y% impact (Scenario 2)
application based on ISO 10874, the technical service + z% impact (Scenario 3)
life recommended by the manufacturer and the with x% + y% + z% = 100%
anticipated strain on the floor by customers, the case-
specific useful life can be established. Based on this
useful life the effects of Module B2 need to be
calculated in order to obtain the overall environmental Name Value Unit
impacts. Collected as mixed construction waste 4.03 kg
4 Environmental Product Declaration Balsan – TAKE A WALK - tufted carpet tiles
(scenario 1 and 2)
Collected separately (scenario 3) 4.03 kg
Landfilling (scenario 1) 4.03 kg
Energy recovery (scenario 2) 4.03 kg
Energy recovery (scenario 3) 1.61 kg
Recycling (scenario 3) 2.42 kg
Reuse, recovery and/or recycling potentials (D),
relevant scenario information
Recovery or recycling potentials due to the three end-
of-life scenarios (module C) are indicated separately.
Recycling in the cement industry (scenario 3)
VDZ e.V.
The organic material of the carpet is used as
secondary fuel in a cement kiln. It mainly substitutes
for lignite (65.5%), hard coal (26.2%) and petrol coke
(8.6%).
The inorganic material is substantially integrated into
the cement clinker and substitutes for original material
input.
5 Environmental Product Declaration Balsan – TAKE A WALK - tufted carpet tiles
LCA: Results
The declared result figures in module B2 have to be multiplied by the assumed service life (in years) of the floor
covering in the building under consideration.
Information on non-relevant modules: Modules B3 - B7 are not relevant during the service life of the carpet.
Modules C1, C3/1, C4/2 and C4/3 cause no additional impact (see chapter "LCA: Calculation rules" in this
document). All these modules are declared and marked as 'modules not relevant/declared'. Module C2 represents
the transport for scenarios 1, 2 and 3. Column D represents module D/A5.
The calculations are based on the CML characterization factors (version August 2016).
DESCRIPTION OF THE SYSTEM BOUNDARY (X = INCLUDED IN LCA; MND = MODULE NOT DECLARED;
MNR = MODULE NOT RELEVANT)
BENEFITS AND
CONSTRUCTI LOADS
PRODUCT STAGE ON PROCESS USE STAGE END OF LIFE STAGE BEYOND THE
STAGE SYSTEM
BOUNDARIES
6 Environmental Product Declaration Balsan – TAKE A WALK - tufted carpet tiles
lairetam
waR
ylppus tropsnarT
gnirutcafunaM
eht
morf
tropsnarT
etis
eht
ot
etag
ylbmessA esU
ecnanetniaM
riapeR
tnemecalpeR tnemhsibrufeR
ygrene
lanoitarepO esu
retaw
lanoitarepO esu
noitcurtsnoc-eD
noitilomed tropsnarT
gnissecorp
etsaW
lasopsiD -esueR -yrevoceR -gnilcyceR laitnetop
A1 A2 A3 A4 A5 B1 B2 B3 B4 B5 B6 B7 C1 C2 C3 C4 D
X X X X X X X MNR MNR MNR MND MND MND X X X X
RESULTS OF THE LCA - ENVIRONMENTAL IMPACT according to EN 15804+A1: 1 m² floorcovering
Parameter Unit A1-A3 A4 A5 B1 B2 C2 C3/2 C3/3 C4/1 D D/1 D/2 D/3
GWP [kg CO2-Eq.] 4.35E+0 2.39E-1 4.20E-1 0.00E+0 2.92E-1 1.34E-2 4.37E+0 4.43E+0 2.74E-1 -1.26E-2 0.00E+0 -3.70E-1 -1.82E-1
-1.80E- -5.20E- -8.62E-
ODP [kg CFC11-Eq.] 7.86E-9 4.18E-172.36E-100.00E+0 1.08E-8 2.34E-181.90E-152.61E-159.29E-16 0.00E+0
16 15 16
AP [kg SO2-Eq.] 1.08E-2 9.90E-4 4.31E-4 0.00E+0 1.08E-3 5.53E-5 2.49E-3 2.67E-3 7.10E-4 -1.40E-5 0.00E+0 -4.07E-4 -4.96E-4
EP [kg (PO4)3--Eq.] 2.14E-3 2.52E-4 9.05E-5 0.00E+0 3.02E-4 1.41E-5 6.08E-4 6.48E-4 7.71E-4 -1.95E-6 0.00E+0 -5.69E-5 -8.54E-5
POCP [kg ethene-Eq.] 9.03E-4 -4.24E-4 1.81E-5 6.29E-5 1.45E-4 -2.37E-5 1.55E-4 9.88E-5 6.39E-5 -1.31E-6 0.00E+0 -3.83E-5 -6.48E-5
ADPE [kg Sb-Eq.] 5.73E-6 2.12E-8 1.78E-7 0.00E+0 2.74E-6 1.19E-9 1.79E-7 1.89E-7 5.25E-8 -2.25E-9 0.00E+0 -6.53E-8 -2.01E-8
ADPF [MJ] 9.78E+1 3.26E+0 3.12E+0 0.00E+0 6.76E+0 1.82E-1 2.56E+0 3.27E+0 4.09E+0 -1.84E-1 0.00E+0-5.40E+0-2.65E+1
GWP = Global warming potential; ODP = Depletion potential of the stratospheric ozone layer; AP = Acidification potential of land and water; EP =
Caption Eutrophication potential; POCP = Formation potential of tropospheric ozone photochemical oxidants; ADPE = Abiotic depletion potential for non-
fossil resources; ADPF = Abiotic depletion potential for fossil resources
RESULTS OF THE LCA - INDICATORS TO DESCRIBE RESOURCE USE according to EN 15804+A1: 1 m²
floorcovering
Parameter Unit A1-A3 A4 A5 B1 B2 C2 C3/2 C3/3 C4/1 D D/1 D/2 D/3
PERE [MJ] 4.04E+1 1.82E-1 2.65E+0 0.00E+0 1.23E+0 1.02E-2 4.49E-1 6.57E-1 3.06E-1 -4.63E-2 0.00E+0 -1.34E+0 -2.11E-1
PERM [MJ] 1.38E+0 0.00E+0 -1.38E+0 0.00E+0 0.00E+0 0.00E+0 0.00E+0 0.00E+0 0.00E+0 0.00E+0 0.00E+0 0.00E+0 0.00E+0
PERT [MJ] 4.18E+1 1.82E-1 1.27E+0 0.00E+0 1.23E+0 1.02E-2 4.49E-1 6.57E-1 3.06E-1 -4.63E-2 0.00E+0 -1.34E+0 -2.11E-1
PENRE [MJ] 7.21E+1 3.27E+0 3.29E+0 0.00E+0 7.85E+0 1.83E-1 3.24E+1 3.33E+1 4.21E+0 -2.21E-1 0.00E+0 -6.48E+0 -2.66E+1
PENRM [MJ] 2.97E+1 0.00E+0 -4.30E-2 0.00E+0 0.00E+0 0.00E+0 -2.96E+1 -2.96E+1 0.00E+0 0.00E+0 0.00E+0 0.00E+0 0.00E+0
PENRT [MJ] 1.02E+2 3.27E+0 3.24E+0 0.00E+0 7.85E+0 1.83E-1 2.82E+0 3.67E+0 4.21E+0 -2.21E-1 0.00E+0 -6.48E+0 -2.66E+1
SM [kg] 8.50E-1 0.00E+0 2.55E-2 0.00E+0 0.00E+0 0.00E+0 0.00E+0 0.00E+0 0.00E+0 0.00E+0 0.00E+0 0.00E+0 1.37E+0
RSF [MJ] 0.00E+0 0.00E+0 0.00E+0 0.00E+0 0.00E+0 0.00E+0 0.00E+0 0.00E+0 0.00E+0 0.00E+0 0.00E+0 0.00E+0 0.00E+0
NRSF [MJ] 0.00E+0 0.00E+0 0.00E+0 0.00E+0 0.00E+0 0.00E+0 0.00E+0 0.00E+0 0.00E+0 0.00E+0 0.00E+0 0.00E+0 0.00E+0
FW [m³] 1.15E-1 2.09E-4 3.89E-3 0.00E+0 4.13E-3 1.17E-5 1.45E-2 1.47E-2 3.88E-5 -4.52E-5 0.00E+0 -1.31E-3 -2.22E-3
PERE = Use of renewable primary energy excluding renewable primary energy resources used as raw materials; PERM = Use of
renewable primary energy resources used as raw materials; PERT = Total use of renewable primary energy resources; PENRE = Use of
non-renewable primary energy excluding non-renewable primary energy resources used as raw materials; PENRM = Use of non-
Caption
renewable primary energy resources used as raw materials; PENRT = Total use of non-renewable primary energy resources; SM = Use
of secondary material; RSF = Use of renewable secondary fuels; NRSF = Use of non-renewable secondary fuels; FW = Use of net fresh
water
RESULTS OF THE LCA – WASTE CATEGORIES AND OUTPUT FLOWS according to EN 15804+A1:
1 m² floorcovering
Parameter Unit A1-A3 A4 A5 B1 B2 C2 C3/2 C3/3 C4/1 D D/1 D/2 D/3
HWD [kg] 1.89E-3 1.65E-10 5.66E-5 0.00E+0 5.90E-10 9.21E-12 5.23E-10 6.51E-10 7.57E-10 -4.91E-11 0.00E+0 -1.44E-9 -1.77E-10
NHWD [kg] 3.33E-1 4.86E-4 4.57E-2 0.00E+0 5.62E-3 2.71E-5 1.19E+0 1.19E+0 4.01E+0 -1.00E-4 0.00E+0 -2.91E-3 -6.23E-4
RWD [kg] 1.54E-3 3.96E-6 4.94E-5 0.00E+0 3.32E-4 2.21E-7 1.02E-4 1.62E-4 4.89E-5 -1.49E-5 0.00E+0 -4.31E-4 -4.51E-5
CRU [kg] 0.00E+0 0.00E+0 0.00E+0 0.00E+0 0.00E+0 0.00E+0 0.00E+0 0.00E+0 0.00E+0 0.00E+0 0.00E+0 0.00E+0 0.00E+0
MFR [kg] 1.12E-2 0.00E+0 9.20E-2 0.00E+0 0.00E+0 0.00E+0 0.00E+0 1.37E+0 0.00E+0 0.00E+0 0.00E+0 0.00E+0 0.00E+0
MER [kg] 0.00E+0 0.00E+0 0.00E+0 0.00E+0 0.00E+0 0.00E+0 0.00E+0 0.00E+0 0.00E+0 0.00E+0 0.00E+0 0.00E+0 0.00E+0
EEE [MJ] 0.00E+0 0.00E+0 1.50E-1 0.00E+0 0.00E+0 0.00E+0 4.79E+0 0.00E+0 0.00E+0 0.00E+0 0.00E+0 0.00E+0 0.00E+0
EET [MJ] 0.00E+0 0.00E+0 2.84E-1 0.00E+0 0.00E+0 0.00E+0 9.08E+0 5.23E+1 0.00E+0 0.00E+0 0.00E+0 0.00E+0 0.00E+0
HWD = Hazardous waste disposed; NHWD = Non-hazardous waste disposed; RWD = Radioactive waste disposed; CRU = Components
Caption for re-use; MFR = Materials for recycling; MER = Materials for energy recovery; EEE = Exported electrical energy; EEE = Exported
thermal energy
Not all of the life cycle inventories applied in this study support the methodological approach for the waste and
water indicators. The data are based on publications of industry. The indicators for waste and water of the system
are evaluated but contain a higher degree of uncertainty.
References
EN 1307 CML characterization factors
DIN EN 1307: 2014+A1:2016+A2:2018-05: Textile Impact assessment characterization factors, version
floor coverings - Classification 4.7, August 2016, Institute of Environmental Sciences -
'Centrum voor Milieuwetenschappen in Leiden' (CML),
EN 13501-1 Leiden, The Netherlands
DIN EN 13501-1:2019-05: Fire classification of
construction products and building elements - Part 1: ECHA candidate list
Classification using data from reaction to fire tests candidate List of substances of very high concern
(SVHCs) for authorisation, 16.01.2020, European
EN 14041 Chemicals Agency (ECHA), Helsinki, Finland
DIN EN 14041: 2018-05: Resilient, textile and laminate
floor coverings - Essential characteristics ecoinvent 3.7
ecoinvent, Zurich, Switzerland, database version 3.7,
EN 15804 published September 2020
EN 15804:2012-04+A1 2013/, Sustainability of
construction works — Environmental Product GaBi database 2021
Declarations — Core rules for the product category of GaBi Software-System and Database for Life Cycle
construction products Engineering, thinkstep AG, Leinfelden-Echterdingen,
2021-2
EN 16810
DIN EN 16810: 2017-08: Resilient, textile and laminate IBU 2021
floor coverings – Environmental product declarations – IBU (2021): General Programme Instructions for the
Product category rules Preparation of EPDs at the Institut Bauen und Umwelt
e.V., Version 2.0 Institut Bauen und Umwelt e.V.,
ISO 10874 Berlin. www.ibu-epd.de
DIN EN ISO 10874: 2012+A1:2021-04: Resilient,
textile and laminate floor coverings - Classification PCR Part A
Product Category Rules for Construction Products
ISO 14025 from the range of Environmental Product Declarations.
DIN EN /ISO 14025:2011-10/, Environmental labels Part A: Calculation Rules for the Life Cycle
and declarations — Type III environmental Assessment and Requirements on the Background
declarations — Principles and procedures Report, V1.9, Berlin: Institut Bauen und Umwelt e.V.
(IBU), January 2021
ISO 14040
DIN EN ISO 14040:2006+A1:2020 Environmental PCR Part B
management - Life cycle assessment - Principles and Product Category Rules for Construction Products
framework from the range of Environmental Product Declarations
of Institut Bauen und Umwelt (IBU),
ISO 14044 Part B: Requirements on the EPD for floor coverings,
DIN EN ISO 14044:2006+A1:2018+A2:2020 V1.2, Berlin: Institut Bauen und Umwelt e.V. (IBU),
Environmental management - Life cycle assessment - February 2018
Requirements and guidelines
PRODIS
ISO 15686 Product Information System (PRODIS) of the
ISO 15686: Buildings and constructed assets - European Carpet Industry, Gemeinschaft
Service life planning umweltfreundlicher Teppichboden e.V (GUT) and
ISO 15686-1: 2011-05: Part 1: General principles and European Carpet and Rug Association
framework (ECRA), http://www.pro-dis.info
ISO 15686-2: 2012-05: Part 2: Service life prediction
procedures REACH
ISO 15686-7: 2017-04: Part 7: Performance Regulation (EC) No 1907/2006 of the European
evaluation for feedback of service life data Parliament and of the Council of 18 December 2006
from practice concerning the Registration, Evaluation, Authorisation
ISO 15686-8: 2008-06: Part 8: Reference service life and Restriction of Chemicals (REACH). Last update:
and service-life estimation 27.02.2020 (Status: 27.06.2018)
Regulation (EU) No. 305/2011 VDZ e.V.
Regulation No. 305/2011 Construction Products Association of German Cement Works, Ed.
Regulation (CPR) of the European Council and of the Environmental Data of the German Cement Industry
European Parliament, April 2011 2019
7 Environmental Product Declaration Balsan – TAKE A WALK - tufted carpet tiles
Publisher
Institut Bauen und Umwelt e.V. Tel +49 (0)30 3087748- 0
Panoramastr. 1 Fax +49 (0)30 3087748- 29
10178 Berlin Mail info@ibu-epd.com
Germany Web www.ibu-epd.com
Programme holder
Institut Bauen und Umwelt e.V. Tel +49 (0)30 - 3087748- 0
Panoramastr 1 Fax +49 (0)30 – 3087748 - 29
10178 Berlin Mail info@ibu-epd.com
Germany Web www.ibu-epd.com
Author of the Life Cycle
Assessment Tel +49 (0)241 96843 410
Gemeinschaft umweltfreundlicher Fax +49 (0)241 96843 400
Teppichboden (GUT) e.V. Mail mail@gut-ev.de
Schönebergstraße 2 Web www.gut-ev.org
52068 Aachen
Germany
Owner of the Declaration
Balsan Moquette Tel +33 (0) 254 2916 00
Corbilly 2 Fax +33 (0) 254 3679 08
36330 Arthon Mail cedric.charton@balsan.com
France Web www.balsan.com
