Environmental Product Declaration (EPD)
According to ISO 14025 and EN 15804
SANCO-tube semi
hard
Registration number: EPD-Kiwa-EE-175077-en
Issue date: 12-06-2024
Valid until: 12-06-2029
Declaration owner: HME Copper Germany GmbH
Publisher: Kiwa-Ecobility Experts
Program operator: Kiwa-Ecobility Experts
Status: verified
SANCO-tube semi hard | ReTHiNK-75077 1 / 18
Environmental Product Declaration
1 General information
Production location:HME Copper Germany GmbH
1.1 PRODUCT Address production location:Carl-Benz-Str. 13, 58706 Menden, DE
SANCO-tube semi hard
1.6 VERIFICATION OF THE DECLARATION
1.2 REGISTRATION NUMBER
The independent verification is in accordance with the ISO 14025:2011. The LCA is in
EPD-Kiwa-EE-175077-en compliance with ISO 14040:2006 and ISO 14044:2006. The EN 15804:2012+A2:2019 serves as
the core PCR.
1.3 VALIDITY Internal ✓ External
Issue date:12-06-2024
Valid until:12-06-2029
1.4 PROGRAM OPERATOR
Kiwa-Ecobility Experts
Wattstraße 11-13
13355 Berlin Lucas Pedro Berman, Senda
DE
1.7 STATEMENTS
The owner of this EPD shall be liable for the underlying information and evidence. The
programme operator Kiwa-Ecobility Experts shall not be liable with respect to
manufacturer data, life cycle assessment data and evidence.
Raoul Mancke Dr. Ronny Stadie
1.8 PRODUCT CATEGORY RULES
(Head of programme operations, Kiwa- (Verification body, Kiwa-Ecobility Experts)
Ecobility Experts)
PCR A: Kiwa-EE General Product Category Rules, Version 2.1, 2022-02-14
PCR B: Requirements on the EPD for Metal pipes for domestic installations, Version 8,
1.5 OWNER OF THE DECLARATION
2023-10-19, From the range of Environmental Product Declarations of Institute
Construction and Environment e.V. (IBU)
Manufacturer:HME Copper Germany GmbH
Address:Carl-Benz-Str. 13, 58706 Menden, DE 1.9 COMPARABILITY
E-mail:info@hmemetal.com
In principle, a comparison or assessment of the environmental impacts of different
Website:https://www.hmemetal.com/
products is only possible if they have been prepared in accordance with EN 15804+A2. For
the evaluation of the comparability, the following aspects have to be considered in
SANCO-tube semi hard | ReTHiNK-75077 2 / 18
Environmental Product Declaration
1 General information
particular: PCR used, functional or declared unit, geographical reference, the definition of Characterization method:EN 15804 +A2 Method v1.0
the system boundary, declared modules, data selection (primary or secondary data,
background database, data quality), scenarios used for use and disposal phases, and the LCA database profiles:EcoInvent version 3.6
life cycle inventory (data collection, calculation methods, allocations, validity period). PCRs Version database:v3.17 (2024-05-22)
and general program instructions of different EPD program operators may differ.
Comparability needs to be evaluated. For further guidance, see EN 15804+A2 (5.3 * Simapro is used for calculating the characterized results of the Environmental profiles
Comparability of EPD for construction products) and ISO 14025 (6.7.2 Requirements for within R<THiNK.
comparability).
1.11 LCA BACKGROUND REPORT
1.10 CALCULATION BASIS
This EPD is generated on the basis of the LCA background report 'SANCO-tube semi hard'
LCA method R<THiNK:Ecobility Experts | EN15804+A2 with the calculation identifier ReTHiNK-75077.
LCA software*:Simapro 9.1
SANCO-tube semi hard | ReTHiNK-75077 3 / 18
Environmental Product Declaration
2 Product
2.1 PRODUCT DESCRIPTION - RAL-Gütezeichen
- ÖVGW QS-G 100, QS-G 313
- ÖVGW QS-W 402, QS-W 100, QS-W 200
This document refers to bare HME SANCO-semi hard copper tubes for domestic
- KIWA BRL-K10018
installations. For the production of those tubes copper Cu-DHP in accordance with DIN
- NF 090
EN1057 is used. Cu-DHP is deoxidised copper with a limited phosphorus content
- AENOR RP 004.01 / AENOR RP 004.03
(maximum 0.04%) which is characterised by its very good weldability and solderability. The
purity is at least 99.90% copper. The dimension range of the copper tubes is between 6
For placing on the market in the EU/EFTA with the exception of Switzerland, Regulation
mm x 0,4 mm and 133 mm x 3,5 mm.
(EU) No. 305/2011 of 9 March 2011 (Construction Product Regulation) applies. The products
require a declaration of performance taking into account the harmonised standard EN
1057:2006+A1:2010 and the CE marking.
Component Share
The respective national regulations apply for use. Planning, processing, commissioning,
Copper ~100% and intended operation of HME branded copper tubes are dependent on the respective
application in accordance to the codes of practice and the manufacturer's
recommendations.
2.2 APPLICATION (INTENDED USE OF THE PRODUCT)
The applications of the declared branded copper tubes are transport of: Descirption Value Unit
• Drinking water cold, warm, circulation Type of metal used Cu - DHP -
• Rainwater
Thermal conductivity of the metal tube 305 W/(mK)
• Heat transfer media in heating, surface heating, surface cooling and solar thermal
energy Coefficient of linear expansion 16.8 (10^-6) (K^-1)
• Refrigerants
Tensile strength 250 N/mm²
• Gas and liquid gas
Elongation at break ≥20 -
2.3 REFERENCE SERVICE LIFE
Modulus of elasticity at 20°C 132 kN/mm²
Density 8.94 g/cm³
RSL PRODUCT
The declared scenarios represent the life cycle stages "Cradle to gate with modules C1–C4 Melting point 1083 °C
and module D". Therefore, according to PCR, no indication of the reference service life is
required. If used according to good engineering practice, no ageing of the products is to
be expected. 2.5 SUBSTANCES OF VERY HIGH CONCERN
USED RSL (YR) IN THIS LCA CALCULATION: No substance present in the product with a contribution of more than 0.10% of the total
50 weight is present on the "List of Potentially Hazardous Substances" (SVHC) that are
candidates for authorisation under REACH legislation.
2.4 TECHNICAL DATA
2.6 DESCRIPTION PRODUCTION PROCESS
SANCO-tubes are manufactured according to:
In the first stage of copper tube production, a pre-tube is produced from the round billet.
- EN 1057 This pre-tube can be produced either by hot forming or by a hot piercing process. Hot
- DVGW GW 392
SANCO-tube semi hard | ReTHiNK-75077 4 / 18
Environmental Product Declaration
2 Product
rolling is followed by cold forming by pilger rolling. This allows high degrees of
deformation. In case of hot forming that process is immediately followed by cold drawing.
The further steps to produce the finished tube are carried out in several stages, each by
cold drawing in drawing machines. In contrast to hot forming, a "flying mandrel" (mandrill)
is used. The respective outer diameter is determined by the die, while the mandrill
determines the inner diameter. The dimension range of the copper tubes is between 6
mm x 0,4 mm and 133 mm x 3,5 mm.
In the course of further processing, HME copper tubes are produced in three different
strength levels. The minimum tensile strength Rm in MPa (N/mm²) is specified as the
characteristic value. This EPD refers to semi-hard copper tubes with a tensile strength of
250 N/mm². The tensile strength of copper is increased during cold forming and can be
reduced again by heating. This means that the strength of semi-hard copper tubes can be
specifically adjusted by intermediate annealing.
SANCO-tube semi hard | ReTHiNK-75077 5 / 18
Environmental Product Declaration
3 Calculation rules
3.1 DECLARED UNIT 3.3 SCOPE OF DECLARATION AND SYSTEM BOUNDARIES
1 kg This is a Cradle to gate with modules C1-C4 and module D LCA. The life cycle stages
The declared unit is 1 kg of SANCO-tubes semi hard. included are as shown below:
(X = module included, ND = module not declared)
Reference unit: kilogram (kg)
A1 A2 A3 A4 A5 B1 B2 B3 B4 B5 B6 B7 C1 C2 C3 C4 D
3.2 CONVERSION FACTORS X X X ND ND ND ND ND ND ND ND ND X X X X X
Description Value Unit
The modules of the EN15804 contain the following:
Reference unit 1 kg
Conversion factor to 1 kg 0.999900 kg Module A1 = Raw material supply Module B5 = Refurbishment
Module A2 = Transport Module B6 = Operational energy use
Module A3 = Manufacturing Module B7 = Operational water use
Module A4 = Transport Module C1 = De-construction / Demolition
Module A5 = Construction -
Module C2 = Transport
Installation process
Module B1 = Use Module C3 = Waste Processing
Module B2 = Maintenance Module C4 = Disposal
Module D = Benefits and loads beyond the
Module B3 = Repair
product system boundaries
Module B4 = Replacement
3.4 REPRESENTATIVENESS
The input data are representative for SANCO-tube semi hard, a product of HME Copper
Germany GmbH. The data are representative for Germany. The scenarios included are
currently in use and are representative for one of the most likely scenario alternatives.
100% scenarios can be given. Additional declaration of representative mixes for the
relevant region is permissible.
3.5 CUT-OFF CRITERIA
Product Stage (A1-A3)
SANCO-tube semi hard | ReTHiNK-75077 6 / 18
Environmental Product Declaration
3 Calculation rules
All input flows (e.g. raw materials, transportation, energy use, packaging, etc.) and output All benefits and loads beyond the system boundary resulting from reusable products,
flows (e.g. production waste) are considered in this LCA. The total neglected input flows do recyclable materials and/or useful energy carriers leaving the product system are
therefore not exceed the limit of 5% of energy use and mass. considered in this LCA.
Furthermore, excluded processes are:
3.6 ALLOCATION
• Manufacturing of equipment used in production, buildings or any other capital asset;
Allocation was avoided where possible. In this LCA study, a physical allocation has been
• Transportation of personnel to the plant;
carried out: The electricity consumption of the production of HME copper tubes has been
• The transportation of personnel within the plant; allocated to 1 kg of product. The differenences in tensile strength of the copper tubes were
neglected. The elctricity consumption of additional processes like annealing in SANCO-
• Research and development activities; tubes semi hard production have been measured.
• Long-term emissions.
3.7 DATA COLLECTION & REFERENCE TIME PERIOD
Construction process stage (A4-A5) All process-specific data was collected for the 2022 operating year. The quantities of raw
materials, consumables and supplies used and the energy consumption were recorded
and averaged over the entire 2022 operating year.
All input flows (e.g. transportation to the construction site, additional raw material use for
construction, installation energy (use)of energy use for assembly , etc.) and output flows
(e.g. construction waste, packaging waste, etc.) are considered in this LCA. The total 3.8 ESTIMATES AND ASSUMPTIONS
neglected input flows do therefore not exceed the limit of 5% of energy use and mass
Representative and average data for Germany was used for most inputs (raw materials and
external inputs). For inputs for which there was no corresponding German data set, a data
Use stage (B1-B3)
set for a neighbouring country (e.g. Switzerland or the Netherlands) or a regional data set
(e.g. for the EU) was used. In a few cases, a global dataset was used. If data was provided by
All (known) input flows (e.g. raw materials, transportation, energy use, packaging, etc.) and a manufacturer (e.g. an EPD), this was used as the data source.
output flows (e.g. emissions to soil, air and water, construction waste, packaging waste,
All specific transport distances of the source materials were recorded and taken into
end-of-life waste, etc.) related to the building fabric are considered in this LCA. The total
account.
neglected input flows do therefore not exceed the limit of 5% of energy use and mass.
The distances from the place of use to the respective waste treatment are taken from the
LCA calculation software R<THiNK, which source for the distances is the National
End of life stage (C1-C4)
Environmental Database (National Environmental Database; NMD) of the Netherlands.
For reasons of data protection, further assumptions are only explained in the background
All input flows (e.g. energy use for demolition or disassembly, transport to waste
report which accompanies this EPD.
processing, etc.) and output flows (e.g. end-of-life waste processing of the product, etc.) are
considered in this LCA. The total neglected input flows do therefore not exceed the limit of A waste scenario for copper has been assumed for Germany. According to the Copper
5% of energy use and mass. Association (Kupferverband), only 10% of the construction waste generated are disposed.
The remaining material was properly recycled and/or reused. More information on this can
be found at Recycling – Kupferverband.
Benefits and Loads beyond the system boundary (Module D)
SANCO-tube semi hard | ReTHiNK-75077 7 / 18
Environmental Product Declaration
3 Calculation rules
The quality of the data used for this EPD can be divided into three categories according to
3.9 DATA QUALITY the criteria of the United Nations Global Environmental Guidelines for the development of
an LCA database (as described in EN 15804+A2).
All process-specific data was collected for the 2022 operating year and is therefore up-to-
date. The data is based on the annual average. In order to ensure comparability of the The quality level of geographical representativeness is very good, the quality level of
results, only consistent background data of the Ecoinvent database V3.6 was used in the technical representativeness can be considered good, and the temporal
LCA (e.g., records on energy, transportation, and supplies), which refers to reference year representativeness can also be considered good. Therefore, the overall data quality for this
2019. The database is regularly reviewed and thus complies with the requirements of EN EPD can be described as good.
15804 (background data not older than 10 years). All consistent datasets contained in the
Ecoinvent database are documented and can be viewed in the online Ecoinvent
3.10 GUARANTEES OF ORIGIN
documentation. The primary data were provided by HME Copper Germany GmbH. The life
cycle was modelled with the R<THiNK EPD App.
In this EPD, the local based approach was considered for the LCA, therefore no guaranties
of origin (GO) are needed.
SANCO-tube semi hard | ReTHiNK-75077 8 / 18
Environmental Product Declaration
4 Scenarios and additional technical information
4.1 DE-CONSTRUCTION, DEMOLITION (C1)
The following information describes the scenario for demolition at end of life.
Description Amount Unit
Diesel, burned in building machine {GLO}| processing | Cut-off, U 0.043 MJ
4.2 TRANSPORT END-OF-LIFE (C2)
The following distances and transport conveyance are assumed for transportation during
end of life for the different types of waste processing.
Waste Scenario Transport conveyance Not removed (stays in work) [km] Landfill [km] Incineration [km] Recycling [km] Re-use [km]
Copper Germany Lorry (Truck), unspecified (default) | market group for (GLO) 0 100 150 50 0
The transport conveyance(s) used in the scenario(s) for transport during end of life has the
following characteristics.
Value and unit
Vehicle type used for transport Lorry (Truck), unspecified (default) | market group for (GLO)
Fuel type and consumption of vehicle not available
Capacity utilisation (including empty returns) 50 % (loaded up and return empty)
Bulk density of transported products inapplicable
Volume capacity utilisation factor 1
4.3 END OF LIFE (C3, C4)
The scenario(s) assumed for end of life of the product are given in the following tables.
First the assumed percentages per type of waste processing are displayed, followed by the
assumed amounts.
Waste Scenario Region Not removed (stays in work) [%] Landfill [%] Incineration [%] Recycling [%] Re-use [%]
Copper Germany DE 0 10 0 90 0
SANCO-tube semi hard | ReTHiNK-75077 9 / 18
Environmental Product Declaration
4 Scenarios and additional technical information
Waste Scenario Not removed (stays in work) [kg] Landfill [kg] Incineration [kg] Recycling [kg] Re-use [kg]
Copper Germany 0.000 0.100 0.000 0.900 0.000
Total 0.000 0.100 0.000 0.900 0.000
4.4 BENEFITS AND LOADS BEYOND THE SYSTEM BOUNDARY (D)
The presented Benefits and loads beyond the system boundary in this EPD are based on
the following calculated Net output flows in kilograms and Energy recovery displayed in
MJ Lower Heating Value.
Waste Scenario Net output flow [kg] Energy recovery [MJ]
Copper Germany 0.374 0.000
Total 0.374 0.000
SANCO-tube semi hard | ReTHiNK-75077 10 / 18
Environmental Product Declaration
5 Results
For the impact assessment, the characterization factors of the LCIA method EN 15804 +A2
Method v1.0 are used. Long-term emissions (>100 years) are not considered in the impact
assessment. The results of the impact assessment are only relative statements that do not
make any statements about end-points of the impact categories, exceedance of threshold
values, safety margins or risks. The following tables show the results of the indicators of the
impact assessment, of the use of resources as well as of waste and other output flows.
5.1 ENVIRONMENTAL IMPACT INDICATORS PER KILOGRAM
CORE ENVIRONMENTAL IMPACT INDICATORS EN15804+A2
Abbr. Unit A1 A2 A3 A1- C1 C2 C3 C4 D
A3
AP mol H+ eqv. 7.33E-2 1.49E-4 2.30E-3 7.57E-2 4.12E-5 4.31E-5 2.69E-4 7.82E-6 -2.74E-2
GWP-total kg CO2 eqv. 1.68E+0 2.07E-2 6.31E-1 2.33E+0 3.94E-3 7.43E-3 2.10E-2 9.39E-4 -6.29E-1
GWP-b kg CO2 eqv. 4.31E-3 6.60E-5 -1.02E-2 -5.83E-3 1.10E-6 3.43E-6 -1.27E-3 4.15E-5 -1.61E-3
GWP-f kg CO2 eqv. 1.68E+0 2.06E-2 6.41E-1 2.34E+0 3.94E-3 7.42E-3 2.22E-2 8.97E-4 -6.27E-1
GWP-luluc kg CO2 eqv. 1.65E-3 1.63E-5 6.24E-4 2.29E-3 3.10E-7 2.72E-6 2.48E-5 2.52E-7 -6.16E-4
EP-m kg N eqv. 6.80E-3 5.23E-5 3.35E-4 7.19E-3 1.82E-5 1.52E-5 5.94E-5 2.89E-6 -2.54E-3
EP-fw kg P eqv. 5.85E-4 5.53E-7 6.57E-5 6.51E-4 1.43E-8 7.49E-8 1.51E-6 1.16E-8 -2.19E-4
EP-T mol N eqv. 1.05E-1 5.79E-4 4.60E-3 1.10E-1 1.99E-4 1.67E-4 6.89E-4 3.20E-5 -3.93E-2
ODP kg CFC 11 eqv. 1.32E-7 3.65E-9 1.35E-7 2.71E-7 8.50E-10 1.64E-9 3.19E-9 3.23E-10 -4.94E-8
kg NMVOC
POCP 2.31E-2 1.60E-4 1.28E-3 2.46E-2 5.48E-5 4.78E-5 1.88E-4 9.14E-6 -8.66E-3
eqv.
ADP-f MJ 2.14E+1 3.07E-1 1.44E+1 3.61E+1 5.42E-2 1.12E-1 3.08E-1 2.40E-2 -8.02E+0
ADP-mm kg Sb-eqv. 1.22E-3 3.37E-7 2.32E-6 1.22E-3 6.04E-9 1.88E-7 1.23E-6 7.88E-9 -4.57E-4
WDP m3 world eqv. 1.46E+0 1.93E-3 8.87E-2 1.56E+0 7.26E-5 4.01E-4 3.10E-3 1.13E-4 -5.48E-1
AP=Acidification (AP) | GWP-total=Global warming potential (GWP-total) | GWP-b=Global warming potential - Biogenic (GWP-b) | GWP-f=Global warming potential - Fossil (GWP-f) | GWP-
luluc=Global warming potential - Land use and land use change (GWP-luluc) | EP-m=Eutrophication marine (EP-m) | EP-fw=Eutrophication, freshwater (EP-fw) | EP-T=Eutrophication,
terrestrial (EP-T) | ODP=Ozone depletion (ODP) | POCP=Photochemical ozone formation - human health (POCP) | ADP-f=Resource use, fossils (ADP-f) | ADP-mm=Resource use, minerals and
metals (ADP-mm) | WDP=Water use (WDP)
SANCO-tube semi hard | ReTHiNK-75077 11 / 18
Environmental Product Declaration
5 Results
ADDITIONAL ENVIRONMENTAL IMPACT INDICATORS EN15804+A2
Abbr. Unit A1 A2 A3 A1- C1 C2 C3 C4 D
A3
ETP-fw CTUe 1.31E+3 3.02E-1 7.53E+0 1.32E+3 3.27E-2 9.98E-2 1.32E+0 1.16E-1 -4.90E+2
PM disease incidence 2.61E-7 1.69E-9 1.16E-8 2.74E-7 1.09E-9 6.68E-10 3.38E-9 1.61E-10 -9.75E-8
HTP-c CTUh 2.86E-8 1.46E-11 1.46E-10 2.88E-8 1.14E-12 3.24E-12 3.22E-11 1.11E-12 -1.07E-8
HTP-nc CTUh 2.08E-6 3.34E-10 4.53E-9 2.09E-6 2.81E-11 1.09E-10 1.53E-9 9.08E-11 -7.78E-7
IR kBq U235 eqv. 1.03E-1 1.51E-3 5.25E-2 1.57E-1 2.32E-4 4.69E-4 1.53E-3 1.20E-4 -3.86E-2
SQP Pt 2.24E+1 2.38E-1 7.32E+0 2.99E+1 6.92E-3 9.71E-2 6.20E-1 5.89E-2 -8.37E+0
ETP-fw=Ecotoxicity, freshwater (ETP-fw) | PM=Particulate Matter (PM) | HTP-c=Human toxicity, cancer (HTP-c) | HTP-nc=Human toxicity, non-cancer (HTP-nc) | IR=Ionising radiation, human
health (IR) | SQP=Land use (SQP)
CLASSIFICATION OF DISCLAIMERS TO THE DECLARATION OF CORE AND ADDITIONAL ENVIRONMENTAL IMPACT INDICATORS
ILCD classification Indicator Disclaimer
Global warming potential (GWP) None
ILCD type / level 1 Depletion potential of the stratospheric ozone layer (ODP) None
Potential incidence of disease due to PM emissions (PM) None
AAcidification potential, Accumulated Exceedance (AP) None
Eutrophication potential, Fraction of nutrients reaching freshwater end compartment
None
(EP-freshwater)
Eutrophication potential, Fraction of nutrients reaching marine end compartment
ILCD type / level 2 None
(EP-marine)
Eutrophication potential, Accumulated Exceedance (EP-terrestrial) None
Formation potential of tropospheric ozone (POCP) None
Potential Human exposure efficiency relative to U235 (IRP) 1
Abiotic depletion potential for non-fossil resources (ADP-minerals&metals) 2
ILCD type / level 3
Abiotic depletion potential for fossil resources (ADP-fossil) 2
Water (user) deprivation potential, deprivation-weighted water consumption (WDP) 2
Potential Comparative Toxic Unit for ecosystems (ETP-fw) 2
SANCO-tube semi hard | ReTHiNK-75077 12 / 18
Environmental Product Declaration
5 Results
ILCD classification Indicator Disclaimer
Potential Comparative Toxic Unit for humans (HTP-c) 2
Potential Comparative Toxic Unit for humans (HTP-nc) 2
Potential Soil quality index (SQP) 2
Disclaimer 1 – This impact category deals mainly with the eventual impact of low dose ionizing radiation on human health of the nuclear fuel cycle. It does not consider effects due to possible
nuclear accidents, occupational exposure nor due to radioactive waste disposal in underground facilities. Potential ionizing radiation from the soil, from radon and from some construction
materials is also not measured by this indicator.
Disclaimer 2 – The results of this environmental impact indicator shall be used with care as the uncertainties on these results are high or as there is limited experienced with the indicator.
5.2 INDICATORS DESCRIBING RESOURCE USE AND ENVIRONMENTAL INFORMATION BASED ON LIFE CYCLE INVENTORY (LCI)
PARAMETERS DESCRIBING RESOURCE USE
Abbr. Unit A1 A2 A3 A1- C1 C2 C3 C4 D
A3
PERE MJ 7.00E+0 1.55E-2 1.24E+0 8.26E+0 2.93E-4 1.40E-3 4.83E-2 1.35E-3 -2.62E+0
PERM MJ 0.00E+0 0.00E+0 3.74E-1 3.74E-1 0.00E+0 0.00E+0 0.00E+0 0.00E+0 0.00E+0
PERT MJ 7.00E+0 1.55E-2 1.61E+0 8.63E+0 2.93E-4 1.40E-3 4.83E-2 1.35E-3 -2.62E+0
PENRE MJ 2.28E+1 3.25E-1 1.52E+1 3.83E+1 5.76E-2 1.19E-1 3.26E-1 2.55E-2 -8.54E+0
PENRM MJ 0.00E+0 0.00E+0 1.84E-1 1.84E-1 0.00E+0 0.00E+0 0.00E+0 0.00E+0 0.00E+0
PENRT MJ 2.28E+1 3.25E-1 1.54E+1 3.85E+1 5.76E-2 1.19E-1 3.26E-1 2.55E-2 -8.54E+0
SM Kg 5.26E-1 0.00E+0 0.00E+0 5.26E-1 0.00E+0 0.00E+0 0.00E+0 0.00E+0 0.00E+0
RSF MJ 0.00E+0 0.00E+0 0.00E+0 0.00E+0 0.00E+0 0.00E+0 0.00E+0 0.00E+0 0.00E+0
NRSF MJ 0.00E+0 0.00E+0 0.00E+0 0.00E+0 0.00E+0 0.00E+0 0.00E+0 0.00E+0 0.00E+0
FW M3 3.70E-2 9.21E-5 4.57E-3 4.16E-2 2.79E-6 1.36E-5 1.46E-4 3.00E-5 -1.38E-2
PERE=renewable primary energy ex. raw materials | PERM=renewable primary energy used as raw materials | PERT=renewable primary energy total | PENRE=non-renewable primary energy
ex. raw materials | PENRM=non-renewable primary energy used as raw materials | PENRT=non-renewable primary energy total | SM=use of secondary material | RSF=use of renewable
secondary fuels | NRSF=use of non-renewable secondary fuels | FW=use of net fresh water
SANCO-tube semi hard | ReTHiNK-75077 13 / 18
Environmental Product Declaration
5 Results
OTHER ENVIRONMENTAL INFORMATION DESCRIBING WASTE CATEGORIES
Abbr. Unit A1 A2 A3 A1- C1 C2 C3 C4 D
A3
HWD Kg 2.66E-5 6.84E-7 1.06E-5 3.79E-5 1.48E-7 2.84E-7 9.27E-7 2.95E-8 -9.97E-6
NHWD Kg 1.30E+0 1.16E-2 3.12E-2 1.35E+0 6.42E-5 7.10E-3 9.00E-3 1.00E-1 -4.87E-1
RWD Kg 9.47E-5 1.94E-6 7.38E-5 1.70E-4 3.76E-7 7.35E-7 1.83E-6 1.59E-7 -3.54E-5
HWD=hazardous waste disposed | NHWD=non hazardous waste disposed | RWD=radioactive waste disposed
ENVIRONMENTAL INFORMATION DESCRIBING OUTPUT FLOWS
Abbr. Unit A1 A2 A3 A1- C1 C2 C3 C4 D
A3
CRU Kg 0.00E+0 0.00E+0 0.00E+0 0.00E+0 0.00E+0 0.00E+0 0.00E+0 0.00E+0 0.00E+0
MFR Kg 0.00E+0 0.00E+0 0.00E+0 0.00E+0 0.00E+0 0.00E+0 9.00E-1 0.00E+0 0.00E+0
MER Kg 0.00E+0 0.00E+0 0.00E+0 0.00E+0 0.00E+0 0.00E+0 0.00E+0 0.00E+0 0.00E+0
EET MJ 0.00E+0 0.00E+0 4.65E-2 4.65E-2 0.00E+0 0.00E+0 0.00E+0 0.00E+0 0.00E+0
EEE MJ 0.00E+0 0.00E+0 2.70E-2 2.70E-2 0.00E+0 0.00E+0 0.00E+0 0.00E+0 0.00E+0
CRU=Components for re-use | MFR=Materials for recycling | MER=Materials for energy recovery | EET=Exported Energy Thermic | EEE=Exported Energy Electric
SANCO-tube semi hard | ReTHiNK-75077 14 / 18
Environmental Product Declaration
5 Results
5.3 INFORMATION ON BIOGENIC CARBON CONTENT PER KILOGRAM
BIOGENIC CARBON CONTENT
The following Information describes the biogenic carbon content in (the main parts of) the
product at the factory gate per kilogram:
Biogenic carbon content Amount Unit
Biogenic carbon content in the product 0 kg C
Biogenic carbon content in accompanying packaging 0.01202 kg C
UPTAKE OF BIOGENIC CARBON DIOXIDE
The following amount carbon dioxide uptake is taken into account. Related uptake and
release of carbon dioxide in downstream processes are not taken into account in this
number although they do appear in the presented results.
Uptake Biogenic Carbon dioxide Amount Unit
Packaging 0.04407 kg CO2 (biogenic)
SANCO-tube semi hard | ReTHiNK-75077 15 / 18
Environmental Product Declaration
6 Interpretation of results
The Raw material supply (A1), and Manufacturing (A3) predominate in almost all of the
environmental impact categories analysed. For example, around 72 % of CO2 emissions
(GWP-total) are attributable to raw material supply, while the A3 module accounts for
around 26 % of the GWP. Copper accounts for approx. 99 % of the total GWP in the raw
material supply (A1) and energy consumption accounts for aprox. 84 % in the
manufacturing (A3).
SANCO-tube semi hard | ReTHiNK-75077 16 / 18
Environmental Product Declaration
7 References
ISO 14040
ISO 14040:2006-10, Environmental management - Life cycle assessment - Principles and
framework; EN ISO 14040:2006
ISO 14044
ISO 14044:2006-10, Environmental management - Life cycle assessment - Requirements
and guidelines; EN ISO 14040:2006
ISO 14025
ISO 14025:2011-10: Environmental labels and declarations — Type III environmental
declarations — Principles and procedures
EN 15804+A2
EN 15804+A2: 2019: Sustainability of construction works — Environmental Product
Declarations — Core rules for the product category of construction products
SANCO-tube semi hard | ReTHiNK-75077 17 / 18
Environmental Product Declaration
8 Contact information
Publisher Operator Owner of declaration
Kiwa-Ecobility Experts Kiwa-Ecobility Experts HME Copper Germany GmbH
Wattstraße 11-13 Wattstraße 11-13 Carl-Benz-Str. 13
13355 Berlin, DE 13355 Berlin, DE 58706 Menden, DE, DE
E-mail: E-mail: E-mail:
DE.Ecobility.Experts@kiwa.com DE.Ecobility.Experts@kiwa.com info@hmemetal.com
Website: Website: Website:
https://www.kiwa.com/de/en/themes/ecobility-experts/ecobility-https://www.kiwa.com/de/en/themes/ecobility-experts/ecobility-https://www.hmemetal.com/
experts-epd-program/ experts-epd-program/
Kiwa-Ecobility Experts is
established member of the
SANCO-tube semi hard | ReTHiNK-75077 18 / 18
