ENVIRONMENTAL PRODUCT DECLARATION
as per ISO 14025 and EN 15804+A2
Owner of the Declaration Kingspan Insulation B.V.
Publisher Institut Bauen und Umwelt e.V. (IBU)
Programme holder Institut Bauen und Umwelt e.V. (IBU)
Declaration number EPD-KIN-20230171-CBA1-EN
Issue date 11/07/2023
Valid to 10/07/2028
Therma™ TW56
Kingspan Insulation B.V.
www.ibu-epd.com | https://epd-online.com
General Information
Kingspan Insulation B.V. Therma™ TW56
Programme holder Owner of the declaration
IBU – Institut Bauen und Umwelt e.V. Kingspan Insulation B.V.
Hegelplatz 1 Lingewei 8
10117 Berlin 4004LL Tiel
Germany Netherlands
Declaration number Declared product / declared unit
EPD-KIN-20230171-CBA1-EN Therma™ TW56
1m2, 40mm thickness, R = 1,40 m2.K/W
D
This declaration is based on the product category rules: Scope:
Insulating materials made of foam plastics, 01/08/2021 The insulation material Therma™ TW56 is produced by Kingspan
(PCR checked and approved by the SVR) Insulation at the manufacturing facility in Kankaanpää (Finland).
Therma™ TW56 is an insulation board with a rigid thermoset
Issue date polyisocyanurate (PIR) fibre-free insulation core, faced on both sides with
a low emissivity composite foil. A plasterboard is adhered to the insulation
11/07/2023
board on one side. Therma™ TW56 is used as thermal insulation for
mechanically fixed and adhesively bonded insulated dry-lining.
Valid to
In order to enable the user of the EPD to calculate the LCA results for
10/07/2028 different thicknesses, the EPD contains the respective calculation rules.
The owner of the declaration shall be liable for the underlying information
and evidence; the IBU shall not be liable with respect to manufacturer
information, life cycle assessment data and evidences.
The EPD was created according to the specifications of EN 15804+A2. In
the following, the standard will be simplified as EN 15804.
Verification
The standard EN 15804 serves as the core PCR
Independent verification of the declaration and data according to ISO
14025:2011
Dipl.-Ing. Hans Peters
(Chairman of Institut Bauen und Umwelt e.V.) internally X externally
Florian Pronold Vito D'Incognito,
(Managing Director Institut Bauen und Umwelt e.V.) (Independent verifier)
1 Environmental Product Declaration - Kingspan Insulation B.V. - Therma™ TW56
Product
The declaration of performance of the product can be found at
Product description/Product definition www.kingspan.com.
ThermaTM TW56 is an insulation board with a rigid thermoset
polyisocyanurate (PIR) fibre-free insulation core, faced on both Base materials/Ancillary materials
sides with a low emissivity composite foil. A plasterboard is The product contains approximately 0,6 kg/m2 polyurethane
adhered to the insulation board. The product is available in 40 rigid foam, 0,3 kg/m2 multi-layer aluminium facings and 6,9
mm and 70 mm thickness. This EPD is based on a thickness of kg/m2 plasterboard.
40 mm and R D-value of 1,40 m²·K/W. The main materials of the polyurethane foam are MDI (between
57-62 %), polyol (between 27-32 %) and a blowing agent
For the placing on the market of the product in the European (between 5-6 %). Due to the closed-cell structure (conform EN
Union/European Free Trade Association (EU/EFTA) (with the 13165), the blowing agent remains in the foam. Water, flame
exception of Switzerland) Regulation (EU) No. 305/2011 (CPR) retardants and additives are added (between 4-8 %).
applies. The product needs a declaration of performance taking In the current REACH regulations, polyurethane foam
into consideration EN 13950 - Gypsum board thermal/acoustic insulation products are considered “articles” and are
insulation composite panels - Definitions, requirements and test exempt from the requirements of Articles 57 and 59(1)
methods and the CE-marking. For the application and use the of REACH Regulation (EC) No 1907/2006. These
respective national provisions apply. products are not classified as “hazardous products”
according to any current legislation, and can hence be
Application declared as follows:
ThermaTM TW56 is used as thermal insulation for mechanically - This article contains substances listed in the
fixed and adhesively bonded insulated dry-lining. candidate list (date: 31.08.2022) exceeding 0.1
percentage by mass: no.
Technical Data
- This article contains other carcinogenic, mutagenic,
Constructional data reprotoxic (CMR) substances in categories 1A or 1B
which are not on the candidate list, exceeding 0.1
Name Value Unit
percentage by mass: no.
Thermal conductivity according to EN 13950 0.022 W(m.K)
- Biocide products were added to this construction
Reaction to fire (plasterboard side) according B- product or it has been treated with biocide products
to EN 13950 s1,d0 (this then concerns a treated product as defined by the
Reaction to fire (PU board side) according to (EU) Biocidal Products Regulation No. 528/2012
F
EN 13950 (BPR): no.
Performance data of the product in accordance with the Reference service life
declaration of performance with respect to its essential
The reference service life is not to be declared in this
characteristics according to EN 13950 - Gypsum board
EPD as it does not cover the use stage.
thermal/acoustic insulation composite panels - Definitions,
requirements and test methods.
LCA: Calculation rules
Declared Unit System boundary
The declared unit (1 m²) and conversion factors are The type of EPD according to EN 15804 is:
listed in the table below. cradle to gate with options, modules C1–C4, and
module D (A1–A3, C, D and additional modules:
Declared unit
A4, A5).
Name Value Unit The product stage is a mandatory information module and it
Declared unit 1 m2 covers:
Gross density of the insulation layer 30 kg/m3 · A1, raw material extraction and processing, processing of
secondary material input (e.g. recycling processes),
Grammage of the plasterboard 6.9 kg/m2
· A2, transport to the manufacturer,
Grammage 7.86 kg/m2 · A3, manufacturing, including provision of all materials,
Layer thickness 0.04 m products and energy, packaging processing and its transport,
as well as waste processing up to the end-of-waste state or
The scope of this EPD is the thermal insulation product
disposal of final residues
Therma™ TW56 as produced by Kingspan Insulation at the
during the product stage.
manufacturing facility in Kankaanpää (Finland). The
environmental impacts have been calculated over the calendar
The construction process stage includes:
year 2021.
· A4 transport to the building site;
· A5 installation in the building including provision of all
The EPD is studied for a product thickness of 40 mm (30mm
materials, products and energy, as well as waste processing up
insulation with a plasterboard adhered to it). Multiplication
to the end-of-waste state or disposal of final residues during the
factors are included to calculate impacts for the product
construction process stage.
thickness of 70 mm (60mm insulation with a plasterboard
adhered to it).
The end-of-life stage is a mandatory information module and it
covers:
2 Environmental Product Declaration - Kingspan Insulation B.V. - Therma™ TW56
· C1 de-construction, demolition;
· C2 transport to waste processing; Comparability
· C3 waste processing for reuse, recovery and/or recycling; Basically, a comparison or an evaluation of EPD data is only
· C4 disposal (not applicable for this EPD) including provision possible if all the data sets to be compared were created
and all transport, provision of all materials, products and related according to EN 15804 and the building context, respectively
energy and water use. the product-specific characteristics of performance, are taken
into account.
Environmental burden of the incineration (R1 > 60 %) of the
product Background database
at the end-of-life stage are assigned to the product system Background data from GaBi ts Version 10 is used with GaBi
(C3); resulting potential credits for thermal and electrical energy data sets CUP2022.1.
from energy substitution are declared in module D.
Period under review
Geographic Representativeness The input data for raw material production and the consumption
Land or region, in which the declared product system is of process energy on the manufacturing facility was measure
manufactured, used or handled at the end of the product´s data during January 1st 2021 to December 31st 2021, i.e.
lifespan: Europe collected over a 12 month period.
LCA: Scenarios and additional technical information
Installation into the building (A5)
Characteristic product properties of biogenic carbon
The total mass of biogenic carbon containing materials is less Name ValueUnit
than 5 % of the total mass of the product and accompanying Output substances following waste treatment on
0.036 kg
packaging. site
The recycling of the packaging is considered in A5.
Technical information
The following technical information is a basis for the End of life (C1-C4)
declared modules or can be used for developing The assumptions for C1 are: diesel driven excavator (100 kW;
specific scenarios in the context of a building 0.2 litre fuel per ton excavated material). The assumptions for
assessment. C2 are: Truck Euro 6, diesel driven, 26-28 t gross weight,
assumed distance 50 km
Manufacturing (A3) Name ValueUnit
A polyethylene packaging foil is used. The products
Collected as mixed construction waste 7.8 kg
are transported on wooden pallets.
Energy recovery 0.875 kg
Within Module A3 the following packaging of the final
Landfilling 6.9 kg
product is included:
- Polyethylene cover and wrap: 0,013 kg/m² Recycling (aluminium content of the multi-layer
0.025 kg
- Expanded Polystyrene skid: 0,000 kg/m² aluminium facings)
- Wooden pallet: 0,023 kg/m²
Reuse, recovery and/or recycling potentials (D), relevant
Transport to the building site (A4) scenario information
Name Value Unit Waste incineration with energy recuperation is assumed as
end-of-life scenario
Litres of fuel 0.0103 l/100km
Transport distance 100 km
Gross density of products transported 195 kg/m3
3 Environmental Product Declaration - Kingspan Insulation B.V. - Therma™ TW56
LCA: Results
DESCRIPTION OF THE SYSTEM BOUNDARY (X = INCLUDED IN LCA; ND = MODULE OR INDICATOR NOT DECLARED; MNR =
MODULE NOT RELEVANT)
Benefits and
Construction loads beyond
Product stage Use stage End-of-life stage
process stage the system
boundaries
la ire ta m w a Ry lp p u s tro p s n a rT g n iru tc a fu n a M e h t m o rf tro p s n a rTe tis e h t o t e ta g y lb m e s s A e s U e c n a n e tn ia M ria p e R tn e m e c a lp e R tn e m h s ib ru fe R y g re n e la n o ita re p Oe s u re ta w la n o ita re p Oe s u n o itc u rts n o c -e Dn o itilo m e d tro p s n a rT g n is s e c o rp e ts a W la s o p s iD -e s u e R-y re v o c e R-g n ilc y c e Rla itn e to p
A1 A2 A3 A4 A5 B1 B2 B3 B4 B5 B6 B7 C1 C2 C3 C4 D
X X X X X MND MND MNR MNR MNR MND MND X X X X X
RESULTS OF THE LCA - ENVIRONMENTAL IMPACT according to EN 15804+A2: 1m2 40mm Therma™ TW56
Parameter Unit A1-A3 A4 A5 C1 C2 C3 C4 D
GWP-total kg CO 2 eq 3.62E+00 6.62E-02 5.34E-02 5.04E-03 3.31E-02 1.97E+00 1.02E-01 -8.98E-01
GWP-fossil kg CO 2 eq 4.25E+00 6.59E-02 2.29E-02 5.04E-03 3.29E-02 1.8E+00 1.04E-01 -8.93E-01
GWP-biogenic kg CO 2 eq -6.31E-01 -9.1E-05 3.05E-02 6.74E-06 -4.55E-05 1.66E-01 -3.03E-03 -4.09E-03
GWP-luluc kg CO 2 eq 2.59E-03 3.67E-04 3.25E-07 6.21E-08 1.84E-04 3.95E-06 3.07E-04 -1.11E-04
ODP kg CFC11 eq 8.57E-12 3.95E-15 6.31E-15 3.09E-16 1.97E-15 1.51E-13 4.05E-16 -4.92E-12
AP mol H+ eq 8.49E-03 6.79E-05 7.15E-06 2.34E-05 3.4E-05 1.11E-03 7.43E-04 -1.88E-03
EP-freshwater kg P eq 1.92E-05 1.97E-07 1.56E-09 1.02E-09 9.84E-08 4.13E-08 1.75E-07 -1.05E-06
EP-marine kg N eq 2.25E-03 2.22E-05 2.18E-06 1.11E-05 1.11E-05 5.31E-04 1.93E-04 -3.63E-04
EP-terrestrial mol N eq 2.32E-02 2.65E-04 3.35E-05 1.22E-04 1.32E-04 6.12E-03 2.12E-03 -3.91E-03
kg NMVOC
POCP 8.54E-03 5.98E-05 6.03E-06 3.16E-05 2.99E-05 1.36E-03 5.85E-04 -1.05E-03
eq
ADPE kg Sb eq 3.31E-06 5.51E-09 1.54E-10 2.06E-10 2.76E-09 4.09E-09 9.85E-09 -1.2E-07
ADPF MJ 9.18E+01 8.81E-01 1.47E-02 6.81E-02 4.4E-01 5.15E-01 1.38E+00 -1.44E+01
m3 world eq
WDP 5.82E-01 5.91E-04 5.32E-03 9.36E-06 2.96E-04 1.98E-01 1.12E-02 -1.05E-01
deprived
GWP = Global warming potential; ODP = Depletion potential of the stratospheric ozone layer; AP = Acidification potential of land and water; EP =
Eutrophication potential; POCP = Formation potential of tropospheric ozone photochemical oxidants; ADPE = Abiotic depletion potential for non-fossil
resources; ADPF = Abiotic depletion potential for fossil resources; WDP = Water (user) deprivation potential)
RESULTS OF THE LCA - INDICATORS TO DESCRIBE RESOURCE USE according to EN 15804+A2: 1m2 40mm Therma™ TW56
Parameter Unit A1-A3 A4 A5 C1 C2 C3 C4 D
PERE MJ 1.73E+01 5.01E-02 2.59E-01 2.57E-04 2.5E-02 9.25E-02 1.86E-01 -4.45E+00
PERM MJ 2.55E-01 0 -2.55E-01 0 0 0 0 0
PERT MJ 1.76E+01 5.01E-02 3.61E-03 2.57E-04 2.5E-02 9.25E-02 1.86E-01 -4.45E+00
PENRE MJ 6.38E+01 8.83E-01 4.02E-01 6.83E-02 4.41E-01 2.82E+01 1.39E+00 -1.44E+01
PENRM MJ 2.8E+01 0 -3.87E-01 0 0 -2.77E+01 0 0
PENRT MJ 9.19E+01 8.83E-01 1.47E-02 6.83E-02 4.41E-01 5.16E-01 1.39E+00 -1.44E+01
SM kg 0 0 0 0 0 0 0 0
RSF MJ 0 0 0 0 0 0 0 0
NRSF MJ 0 0 0 0 0 0 0 0
FW m3 2.74E-02 5.66E-05 1.26E-04 3.88E-07 2.83E-05 4.66E-03 3.42E-04 -6.08E-03
PERE = Use of renewable primary energy excluding renewable primary energy resources used as raw materials; PERM = Use of renewable primary
energy resources used as raw materials; PERT = Total use of renewable primary energy resources; PENRE = Use of non-renewable primary energy
excluding non-renewable primary energy resources used as raw materials; PENRM = Use of non-renewable primary energy resources used as raw
materials; PENRT = Total use of non-renewable primary energy resources; SM = Use of secondary material; RSF = Use of renewable secondary fuels;
NRSF = Use of non-renewable secondary fuels; FW = Use of net fresh water
RESULTS OF THE LCA – WASTE CATEGORIES AND OUTPUT FLOWS according to EN 15804+A2:
1m2 40mm Therma™ TW56
Parameter Unit A1-A3 A4 A5 C1 C2 C3 C4 D
HWD kg 4.74E-08 4.23E-12 1.31E-12 2.26E-13 2.11E-12 6.91E-11 1.47E-10 -1.33E-09
NHWD kg 4.91E-01 1.27E-04 2.24E-03 6.39E-06 6.33E-05 1.44E-02 6.91E+00 -6.06E-02
RWD kg 1.93E-03 1.09E-06 7.22E-07 7.48E-08 5.44E-07 2.2E-05 1.45E-05 -1.1E-03
CRU kg 0 0 0 0 0 0 0 0
MFR kg 0 0 0 0 0 2.54E-02 0 0
MER kg 0 0 2.6E-02 0 0 8.15E-01 0 0
EEE MJ 0 0 8.53E-02 0 0 3.11E+00 0 0
EET MJ 0 0 1.53E-01 0 0 5.56E+00 0 0
HWD = Hazardous waste disposed; NHWD = Non-hazardous waste disposed; RWD = Radioactive waste disposed; CRU = Components for re-use;
MFR = Materials for recycling; MER = Materials for energy recovery; EEE = Exported electrical energy; EET = Exported thermal energy
4 Environmental Product Declaration - Kingspan Insulation B.V. - Therma™ TW56
RESULTS OF THE LCA – additional impact categories according to EN 15804+A2-optional:
1m2 40mm Therma™ TW56
Parameter Unit A1-A3 A4 A5 C1 C2 C3 C4 D
Disease
PM 1.14E-07 3.92E-10 5.56E-11 2.65E-10 1.96E-10 3.2E-09 9.23E-09 -1.76E-08
incidence
IR kBq U235 eq 2.62E-01 1.59E-04 1.09E-04 1.09E-05 7.97E-05 3.52E-03 1.52E-03 -1.91E-01
ETP-fw CTUe 3.64E+01 6.12E-01 8.75E-03 4.74E-02 3.06E-01 1.83E-01 7.89E-01 -3.5E+00
HTP-c CTUh 2.43E-09 1.23E-11 5.24E-13 8.77E-13 6.16E-12 1.33E-11 1.16E-10 -2.35E-10
HTP-nc CTUh 2.04E-07 6.4E-10 4.04E-11 4.44E-11 3.2E-10 4.92E-10 1.28E-08 -6.98E-09
SQP SQP 4.48E+01 3.03E-01 4.01E-03 1.88E-04 1.52E-01 1.12E-01 2.8E-01 -2.22E+00
PM = Potential incidence of disease due to PM emissions; IR = Potential Human exposure efficiency relative to U235; ETP-fw = Potential comparative
Toxic Unit for ecosystems; HTP-c = Potential comparative Toxic Unit for humans (cancerogenic); HTP-nc = Potential comparative Toxic Unit for humans
(not cancerogenic); SQP = Potential soil quality index
Disclaimer 1 – for the indicator 'Potential Human exposure efficiency relative to U235'.This impact category deals mainly with the
eventual impact of low-dose ionizing radiation on human health of the nuclear fuel cycle. It does not consider effects due to possible
nuclear accidents, occupational exposure or to radioactive waste disposal in underground facilities. Potential ionizing radiation from the
soil, radon and from some construction materials is also not measured by this indicator.
Disclaimer 2 – for the indicators 'abiotic depletion potential for non-fossil resources', 'abiotic depletion potential for fossil resources',
'water (user) deprivation potential, deprivation-weighted water consumption', 'potential comparative toxic unit for ecosystems', 'potential
comparative toxic unit for humans – cancerogenic', 'Potential comparative toxic unit for humans - not cancerogenic', 'potential soil
quality index'. The results of this environmental impact indicator shall be used with care as the uncertainties on these results are high
as there is limited experience with the indicator.
Factors for different thicknesses
The LCA results for the insulation material declared in this EPD refer to a product with a thickness of 40 mm. To enable the user of the
EPD to calculate the results for a product thickness of 70 mm the factors in the following table can be used for the calculation. The LCA
results in chapter 5 have to be multiplied with these factors.
This EPD was created using a software tool.
References
Biocidal Products Regulation No. 528/2012 (BPR) 89/106/EC
Regulation (EU) No 528/2012 of the European
Parliament and of the Council of 22 May 2012 ISO 14025
concerning the making available on the market and EN ISO 14025:2011, Environmental labels and
use of biocidal products declarations — Type III environmental declarations —
Principles and procedures.
CPR
Regulation (EU) No. 305/2011 of the European EN 13165
Parliament and of the Council of 9 March 2011 laying EN 13165:2012+A2:2016: Thermal insulation products
down harmonised condition for the marketing of for buildings. Factory made polyurethane foam (PU)
construction products and repealing Council Directive products. Specification
5 Environmental Product Declaration - Kingspan Insulation B.V. - Therma™ TW56
EN 13950 PCR Version 1.7, Part A
EN 13950:2014: Gypsum board thermal/acoustic insulation Institut Bauen und Umwelt e.V., Berlin (pub.): Product
composite panels - Definitions, requirements and test methods Category Rules for Building-Related Products and
services, Part A: Calculation Rules for the Life Cycle
EN 15804 Assessment and Requirements on the Project Report
EN 15804:2012+A2:2019+AC:2021, Sustainability of according to EN 15804+A2:2019
construction works — Environmental Product November 2021
Declarations — Core rules for the product category of
construction products. PCR 2023, Part B
Institut Bauen und Umwelt e.V., Berlin (pub.): Product
GaBi ts Category Rules for Construction Products from the
thinkstep AG: Leinfelden-Echterdingen GaBi Software- range of Environmental Product Declarations of Institut
System and Database for Life Cycle Engineering 1992- Bauen und Umwelt (IBU), Part B: Requirements on the
2019 EPD for insulating materials made of foam
plastics. May 2023
IBU 2022
Institut Bauen und Umwelt e.V.: General Instructions REACH
for the EPD programme of Institut Bauen und Umwelt Regulation (EC) No 1907/2006 of the European
e.V., Version 2.1, Berlin: Institut Bauen und Umwelt Parliament and of the Council on the Registration,
e.V., 2022. Evaluation, Authorisation and Restriction of Chemicals
www.ibu-epd.com (REACH)
https://echa.europa.eu/candidate-list-table;
LCA-tool
Kingspan LCA tool, version 1.1. IBU-KSI-202001-LT1- Candidate list
EN. https://echa.europa.eu/candidate-list-table; accessed
Developed by Sphera Solutions GmbH (formely 31.08.2022, 233 substances listed.
Thinkstep GmbH)
6 Environmental Product Declaration - Kingspan Insulation B.V. - Therma™ TW56
Publisher
Institut Bauen und Umwelt e.V. +49 (0)30 3087748- 0
Hegelplatz 1 info@ibu-epd.com
10117 Berlin www.ibu-epd.com
Germany
Programme holder
Institut Bauen und Umwelt e.V. +49 (0)30 3087748- 0
Hegelplatz 1 info@ibu-epd.com
10117 Berlin www.ibu-epd.com
Germany
Author of the Life Cycle Assessment
Kingspan Insulation B.V. +31 (0) 543 543 210
Lingewei 8 info@kingspaninsulation.nl
4004LL Tiel www.kingspan.com
Netherlands
Owner of the Declaration
Kingspan Insulation B.V. +31 (0) 543 543 210
Lingewei 8 info@kingspaninsulation.nl
4004LL Tiel www.kingspan.com
Netherlands
7 Environmental Product Declaration - Kingspan Insulation B.V. - Therma™ TW56
