ENVIRONMENTAL PRODUCT DECLARATION
as per ISO 14025 and EN 15804+A2
Owner of the Declaration ARGE – The European Federation of Locks and Building Hardware Manufacturers
Publisher Institut Bauen und Umwelt e.V. (IBU)
Programme holder Institut Bauen und Umwelt e.V. (IBU)
Declaration number EPD-ARG-20230540-IBG1-EN
Issue date 02.04.2024
Valid to 01.04.2029
Window fittings
ARGE – The European Federation of Locks
and Building Hardware Manufacturers
This EPD is valid only for products supplied by an ARGE EPD licence holder.
www.ibu-epd.com | https://epd-online.com
1. General Information
ARGE – The European Federation of Locks Window fittings
and Building Hardware Manufacturers
Programme holder Owner of the declaration
IBU – Institut Bauen und Umwelt e.V. ARGE – The European Federation of Locks and Building Hardware
Hegelplatz 1 Manufacturers
10117 Berlin Offerstraße 12
Germany 42551 Velbert
Germany
Declaration number Declared product / declared unit
EPD-ARG-20230540-IBG1-EN 1 kg of window fitting
This declaration is based on the product category rules: Scope:
Building Hardware products, 01.08.2021 This ARGE EPD covers window fittings designed to be integrated into
(PCR checked and approved by the SVR) window assemblies of varying materials and applications. The reference
product used to calculate the impact this product group has on the
environment is a window fitting composed primarily of Zinc, aluminium and
Issue date steel and has been selected for the LCA (Life Cycle Assessment) because
it is the product with the highest impact for 1 kg of product. A validity scope
02.04.2024
analysis has also been carried out to determine the limiting factors for
window fittings covered by this EPD. In a preliminary study (simplified
LCA), it has been confirmed that this EPD represents the worst-case
Valid to
condition and it can therefore be used to cover all window fittings
01.04.2029 manufactured in Europe by ARGE member companies.
The owner of the declaration shall be liable for the underlying information
and evidence; the IBU shall not be liable with respect to manufacturer
information, life cycle assessment data and evidences.
The EPD was created according to the specifications of EN 15804+A2. In
the following, the standard will be simplified as EN 15804.
Verification
The standard EN 15804 serves as the core PCR
Independent verification of the declaration and data according to ISO
14025:2011
Dipl.-Ing. Hans Peters
(Chairman of Institut Bauen und Umwelt e.V.) internally X externally
Florian Pronold Dr. Matthew Fishwick,
(Managing Director Institut Bauen und Umwelt e.V.) (Independent verifier)
1 Environmental Product Declaration - ARGE – The European Federation of Locks and Building Hardware Manufacturers - Window fittings
2. Product
other elements depending on the desired characteristics.
2.1 Product description/Product definition
Components made of steel are formed by stamping or other
This EPD refers to mechanisms that allow the opening and types of mechanical processing.
closing of windows and have a range of actions (e.g., pivoting,
sliding, tilt and turn, etc.). It covers products with different raw Aluminium is a non-ferrous metal produced from bauxite by
material compositions and different designs. For the application the Bayer process. Components made of aluminium are
and use the respective national provisions apply. manufactured by extrusion or other types of mechanical
processing.
2.2 Application
These products are designed to be integrated into window Stainless steel is produced by combining iron with chromium
assemblies consisting of various materials and used for various as well as other elements depending on the desired
applications. Their purpose is to ensure the correct functionality characteristics. Components made of steel are formed by
of the window. They may be used for either interior or exterior stamping or other types of mechanical processing.
windows.
Nylon 66 is a polymer, in particular polyamide. It is formed by
2.3 Technical Data
the polycondensation of hexamethylenediamine and adipic acid
Ideally, products should comply with a suitable technical
in equal parts. Components made of Nylon 66 are formed by
specification. EN 13126, parts 1-19, various publication dates,
injection moulding or other thermal forming processes.
Building hardware – Requirements and test methods for
windows and door height windows, is an example of such a
ABS (acrylonitrile butadiene styrene) is a terpolymer polymer
specification and some products will comply with it. The
made by polymerizing styrene and acrylonitrile in the presence
relevant grading structure is shown in the following table:
of polybutadiene. Components made of ABS are made by
Name Value Unit
injection moulding or other thermal forming processes.
Category of use - Grade
Durability H1, H2, H3 (3, 4, 5) Grade PEHD (polyethylene high-density) is a thermoplastic polymer
Sash mass - Grade produced from the monomer ethylene. Components made of
PEHD are formed by injection moulding or other thermal
Fire resistance 0 Grade
forming processes.
Safety 1 Grade
Corrosion resistance 2, 3, 4 Grade Nylon 6 is a polymer, in particular polyamide. It is formed by
the ring-opening polymerisation of caprolactam. Components
Performance data of the product in respect to its characteristics
made of Nylon 6 are formed by injection moulding or other
in accordance with the relevant technical provision (no CE-
thermal forming processes.
marking).
2.4 Delivery status PP (polypropylene) is a thermoplastic polymer produced from
The products are sold by unit. Deliveries of individual items are propylene by a polymerisation process. Components made of
possible but are an exception. Standard deliveries comprise a PP are formed by injection moulding or other thermal forming
larger quantity of window fittings, as they are marketed as processes.
"B2B" products and not to end-users.
Zamak is an alloy with a base metal of zinc and alloying
2.5 Base materials/Ancillary materials elements of aluminium, magnesium, and copper. Components
Composition of product analysed for this EPD: made of Zamak are die-cast.
The values given in the table below are for the product ASA (acrylonitrile styrene acrylate), also called acrylic
analysed for this EPD. Ranges of the values for other products styrene acrylonitrile, is an amorphous thermoplastic, specifically
covered by the validity scope analysis are shown in brackets. an acrylate rubber-modified styrene acrylonitrile copolymer.
Name Value Unit Components made of ASA are formed by injection moulding or
other thermal forming processes.
Zinc (0.00% – 59.19%) 59.19 %
Steel (19.43% – 91.01%) 19.43 %
1) This product/article/at least one partial article contains
Aluminium (0.00% – 19.22%) 19.22 % substances listed in the ECHA candidate list (date: 14.06.2023)
Stainless steel (0.00% – 6.60%) 0.82 % exceeding 0.1 percentage by mass: Certain components may
Nylon 66 (0.67% – 5.23%) 1.34 % contain small amounts of lead (CAS no. 7439-92-1) as an
alloying element.
ABS (0.00% – 0.06%) 0 %
PEHD (0.00% – 0.75%) 0 %
2) This product/article/at least one partial article contains other
Nylon 6 (0.00% – 0.10%) 0 % cancerogenic, mutagenic, reprotoxic (CMR) substances in
PP (0.00% – 0.13%) 0 % categories 1A or 1B which are not on the ECHA candidate list,
Zamak (0.00% – 10.79%) 0 % exceeding 0.1 percentage by mass: no.
ASA (0.00% – 0.21%) 0 %
3) Biocide products were added to this construction product or it
has been treated with biocide products (this then concerns a
Zinc is a slightly brittle metal. Zinc metal is produced using treated product as defined by the (EU) Ordinance on Biocide
extractive metallurgy. The components made of zinc are die- Products No. 528/2012): no.
cast.
2.6 Manufacture
Steel is produced by combining iron with carbon as well as
2 Environmental Product Declaration - ARGE – The European Federation of Locks and Building Hardware Manufacturers - Window fittings
The manufacture of a window fitting ususally follows a 3-step No environmental damage or health risks are to be expected
process: during normal conditions of use.
1. Manufacture of the components: this step may include
2.12 Reference service life
surface treatment in the factory or by external
The reference service life is 30 years under normal working
contractors.
conditions. This corresponds to passing a mechanical
2. Pre-assembly of modules (in the factory).
endurance test of 25.000 cycles as specified in the EN 13126.
3. Final assembly (in the factory).
The reference service life is dependent on the actual frequency
2.7 Environment and health during manufacturing of use and environmental conditions. It is required that
Regular measurements of air quality and noise levels are installation, as well as maintenance of the product, must be
done in line with instructions provided by the manufacturer.
carried out by the manufacturers, the ARGE member
companies. The results shall be within the mandatory safety
2.13 Extraordinary effects
levels. In areas where employees are exposed to chemical
Fire
products, the required protective clothing and technical
There are no specific fire resistance requirements.
protective devices shall be provided. Regular health checks are
mandatory for employees in production facilities.
Water
2.8 Product processing/Installation The declared product is intended to be used in buildings under
normal conditions (indoor or outdoor use). The product shall not
The installation of the product may vary depending on the type
emit hazardous substances in the event of flooding.
of window and the specific situation, but the products shall not
require energy consumption for installation.
Mechanical destruction
2.9 Packaging Mechanical destruction of the declared product shall not
Normally, each individual product is packed in paper or materially alter its composition or have any adverse effect on
cardboard. These individual products are then packed in a the environment.
cardboard box and stacked on wooden pallets for transport to
2.14 Re-use phase
the customer.
Removal of window fittings (for re-use or recycling) shall have
no adverse effect on the environment.
Waste from product packaging is collected separately for waste
disposal (including recycling).
2.15 Disposal
2.10 Condition of use Window fittings should be recycled wherever possible,
providing that there is no adverse effect on the environment.
Once installed, the products shall require no servicing during
The waste code in accordance with the European Waste Code
their expected service lives. There shall be no consumption of
is 17 04 07.
water or energy linked to their use, and they shall not cause
any emissions.
2.16 Further information
2.11 Environment and health during use Details of all types and variants can be found on the
manufacturers' websites. The respective website addresses are
available at https://arge.org.
3. LCA: Calculation rules
their transformation process is taken into account and not the
3.1 Declared Unit
extraction of the raw material.
The declared unit for all products covered by ARGE EPD is 1 A4 module represents the transport of the finished window
kg (of product). Since individual products will rarely weigh fittings to the installation site.
exactly 1 kg it is necessary to establish the exact weight of the There is no waste associated with the installation of the
product and then use this as a correction factor to determine product. The A5 module therefore represents only the disposal
the actual values for 1 kg of product in the tables (Section 5). of the product packaging.
Declared unit The end-of-Life (EoL) stages are also considered. The
transportation to the EoL disposal site is taken into account in
Name Value Unit
module C2. Module C4 covers the disposal of the locks. Module
Declared unit 1 kg
C3 covers the recycling of the individual elements according to
Mass of declared product 1.47 kg European averages, with the remaining waste divided between
Raw density 1 kg/m3 incineration and landfill. Such a mixed scenario is declared due
to the complex material mix of the product and the dependency
of the EoL-route on the EoL-route of the product the window
3.2 System boundary
fittings have been integrated into.
Type of the EPD: "cradle to gate with options, with modules C1
In practice, the end of life has been modelled as follows:
– C4, and module D (A1-A3, C1-C3, D and additional
modules)" • when a material is sent for recycling, generic transport
and electric consumption of a shredder is taken into
The analysis of the product life cycle includes the production account (corresponding to the process 'Grinding,
and transport of the raw materials, the manufacture of the metals'). Only then, is the material considered to have
product and the packaging materials which are declared in attained the 'end-of-waste' state.
modules A1-A3. • each type of waste is modelled as a transport to the
Losses during production are considered as waste and are sent treatment site with a distance of 30 km. Parts sent for
for recycling. No recycling processes are taken into account recycling include electricity consumption (grinding) and
except for transport and electricity consumption for grinding the a flow ('Materials for recycling, unspecified').
metals. When recycled metals are used as raw material only
3 Environmental Product Declaration - ARGE – The European Federation of Locks and Building Hardware Manufacturers - Window fittings
2022).
3.3 Estimates and assumptions • In the absence of collected data, generic data from the
The LCA data of the declared window fittings had been ecoinvent v3.8 database has been used. This is updated
calculated from the production data of one ARGE member regularly and is representative of current processes (the
company, representing 3 different products. This company had entire database having been updated in 2021).
been chosen by ARGE as being representative by means of its Geography: Data come from a production site of the ARGE
production processes and its market share. The window fittings member company. Generic data come from the ecoinvent
chosen as representative for this calculation follow the "worst- database, representative for European production processes.
case" principle as explained under section 6. LCA
interpretation. Technology: Material shaping technologies are based on
European technology in the case of the use of generic data.
3.4 Cut-off criteria
The cut-off criteria considered are 1% of renewable and non- A total of 3 typical products (based on sales figures) have been
renewable primary energy usage and 1% of the total mass of evaluated, and the worst-case results are used in the tables.
that unit process. The total neglected input flows per module
shall be a maximum of 5% of energy usage and mass. 3.7 Period under review
The data of the LCA is based on the annual production data of
For this study, all input and output flows have been considered an ARGE member from 2013, considered representative for the
at 100%, including raw materials as per the product year 2022.
composition provided by the manufacturer and packaging of
raw materials as well as the final product. Energy and water 3.8 Geographic Representativeness
consumptions have also been considered at 100% according to Land or region, in which the declared product system is
the data provided. manufactured, used or handled at the end of the product´s
lifespan: Europe
With the approach chosen, no significant environmental
impacts are known to have been cut off.
3.9 Allocation
3.5 Background data The products covered by this EPD are produced in one
For the life cycle modelling of the considered product, all production site. All data were provided by the manufacturer of
relevant background datasets are taken from ecoinvent v3.8 the products per unit and then divided by the mass of the
(system model: cut-off by classification). product to give a value per kg of product produced.
3.6 Data quality The assumptions relating to the EoL of the product are
The objective of this evaluation is to evaluate the environmental described in the section System Boundaries.
impacts generated by the products throughout their entire life
cycles. To this end, ISO 14040, ISO 14044 and EN 15804 have 3.10 Comparability
been met regarding the quality of data on the following different Basically, a comparison or an evaluation of EPD data is only
criteria: possible if all the data sets to be compared were created
according to EN 15804 and the building context, respectively
Time: The life cycle inventory data used come from: the product-specific characteristics of performance, are taken
into account.
• Data collected specifically for this study on the ARGE
ecoinvent v3.8 (system model: cut-off by classification) has
member company's manufacturing site. Datasets are
been used as the background database.
based on 1-year averaged data (time period: January
2013 to December 2013 considered representative for
4. LCA: Scenarios and additional technical information
Name Value Unit
Characteristic product properties of biogenic carbon
Material loss 0.144 kg
Information on the biogenic carbon content at factory gate
Note: 1 kg of biogenic carbon is equivalent to 44/12 kg of CO . Reference service life
2
Name Value Unit
Name Value Unit
Reference service life 30 a
kg
Biogenic carbon content in product 0 C Test cycles over RSL (EN 13126) 25'000 cycles
Biogenic carbon content in accompanying kg
0.0570 End of life (C1-C4)
packaging C
Name Value Unit
Collected separately waste type 1 kg
The following information is the basis of the declared modules
Recycling 0.317 kg
within the LCA in this EPD.
Energy recovery 0.314 kg
Transport to the building site (A4)
Landfilling 0.369 kg
Name Value Unit
It is assumed that a 16–32-ton truck is used to transport the
Litres of fuel 25.8 l/100km
product:
Transport distance 3500 km
- Transport to shredding facility for metal recovery: 150 km
Capacity utilisation (including empty runs) 36 % - Transport to municipal waste incineration plant: 50 km
- Transport to landfill: 30 km
Installation into the building (A5)
4 Environmental Product Declaration - ARGE – The European Federation of Locks and Building Hardware Manufacturers - Window fittings
Reuse, recovery and/or recycling potentials (D), relevant recycling (MFR);
scenario information - net amounts of a metal leaving the product system are
quantified as the material for recycling leaving modules A1-C4
Module D contains the benefits and loads beyond the system minus the input of secondary scrap (secondary material, SM) to
boundary related to the recycling of metals, which result from the product system
the treatment of recycled materials from the point of end-of- - in the case of brass and zinc alloys, which are composed of
waste status to the point of substitution (as costs) and the two different constituting metals, no difference shall be made
substitution of primary resources (as benefits). between the input of secondary constituting metals (Cu and Zn;
Cu and Sn) and its alloys (CuZn; CuSn).
According to EN 16710, clause 6.4.3.3: 'In module D
substitution effects are calculated only for the resulting net Negative net output flows have not been considered in the
output flow. quantification of module D.
For building hardware, the following rules apply for the It also includes the benefits and loads related to 'exported
quantification of net output flows: energy electricity' and 'exported energy heat' resulting from the
- all production scrap and cuttings leave modules A1-B3 as energy recovery from plastic wastes in a municipal waste
sorted scrap without allocated burdens from primary production; incineration plant as modelled in Modules A3, A5 and C4.
the corresponding amounts are declared as material for
5 Environmental Product Declaration - ARGE – The European Federation of Locks and Building Hardware Manufacturers - Window fittings
5. LCA: Results
In Table 1 "Description of the system boundary", the declared modules are indicated with an "X"; all modules that are not declared
within the EPD but where additional data are available are indicated with "MND". Those data can also be used for building assessment
scenarios. The values are declared with three valid digits in exponential form. The set of characterisation factors EF3.0 has been used
for the life cycle assessment.
DESCRIPTION OF THE SYSTEM BOUNDARY (X = INCLUDED IN LCA; MND = MODULE OR INDICATOR NOT DECLARED; MNR
= MODULE NOT RELEVANT)
Benefits and
Construction loads beyond
Product stage Use stage End of life stage
process stage the system
boundaries
la ire wta am R y lp p u s tro p s n a rT g n iru tc a fu n a M tro p s nm ae o rh r
T
f te tis e h t o t e ta g y lb m e s s A e s U e c n a n e tn ia M ria p e R tn e m e c a lp e R tn e m h s ib ru fe R la n o ity ag rr ee pn Oe e s u la n o ita r re et pa Ow e s u n o itc u rts n eo Dc -n o itilo m e d tro p s n a rT g n is s ee tsc ao Wrp la s o p s iD e s u e R- y re v o c e R- g n ilc y c e R- la itn e to p
A1 A2 A3 A4 A5 B1 B2 B3 B4 B5 B6 B7 C1 C2 C3 C4 D
X X X X X MND MND MNR MNR MNR MND MND X X X X X
RESULTS OF THE LCA - ENVIRONMENTAL IMPACT according to EN 15804+A2: 1 kg of window fittings
Parameter Unit A1-A3 A4 A5 C1 C2 C3 C4 D
GWP-total kg CO2 eq 1.1E+01 6.52E-01 2.32E-01 0 1.54E-02 3.28E-03 1.95E-02 -4.94E+00
GWP-fossil kg CO2 eq 1.12E+01 6.52E-01 2.33E-02 0 1.54E-02 3.27E-03 1.95E-02 -4.93E+00
GWP-biogenic kg CO2 eq -2.09E-01 0 2.09E-01 0 0 0 0 0
GWP-luluc kg CO2 eq 2.7E-02 2.61E-04 1.24E-06 0 6.15E-06 8.16E-06 3.48E-06 -1.53E-02
ODP kg CFC11 eq 5.93E-07 1.51E-07 6.91E-10 0 3.56E-09 1.66E-10 1.3E-09 -1.74E-07
AP mol H+ eq 8.63E-02 1.85E-03 1.72E-05 0 4.37E-05 1.68E-05 3.48E-05 -3.67E-02
EP-freshwater kg P eq 5.15E-04 4.65E-06 2.96E-08 0 1.1E-07 3.67E-07 7.34E-08 -2.23E-04
EP-marine kg N eq 1.3E-02 3.68E-04 6.11E-06 0 8.67E-06 2.16E-06 1.29E-05 -4.98E-03
EP-terrestrial mol N eq 1.39E-01 4.1E-03 6.6E-05 0 9.67E-05 2.5E-05 1.33E-04 -5.56E-02
kg NMVOC
POCP 4.21E-02 1.58E-03 1.85E-05 0 3.72E-05 6.82E-06 3.97E-05 -1.75E-02
eq
ADPE kg Sb eq 1.37E-03 2.31E-06 1.14E-08 0 5.45E-08 7.92E-09 1.74E-08 -5.45E-04
ADPF MJ 1.21E+02 9.89E+00 4.76E-02 0 2.33E-01 6.93E-02 9.47E-02 -4.64E+01
m3 world eq
WDP 2.63E+00 3.01E-02 3E-04 0 7.09E-04 7.74E-04 -9.77E-04 -9.12E-01
deprived
GWP = Global warming potential; ODP = Depletion potential of the stratospheric ozone layer; AP = Acidification potential of land and water; EP =
Eutrophication potential; POCP = Formation potential of tropospheric ozone photochemical oxidants; ADPE = Abiotic depletion potential for non-fossil
resources; ADPF = Abiotic depletion potential for fossil resources; WDP = Water (user) deprivation potential)
RESULTS OF THE LCA - INDICATORS TO DESCRIBE RESOURCE USE according to EN 15804+A2: 1 kg of window fittings
Parameter Unit A1-A3 A4 A5 C1 C2 C3 C4 D
PERE MJ 1.34E+01 1.39E-01 -7.08E-01 0 3.28E-03 1.31E-02 3.96E-03 -5.94E+00
PERM MJ 1.78E+00 0 -2.15E-01 0 0 0 0 0
PERT MJ 1.51E+01 1.39E-01 -9.23E-01 0 3.28E-03 1.31E-02 3.96E-03 -5.94E+00
PENRE MJ 1.21E+02 9.89E+00 3.38E-01 0 2.33E-01 6.99E-02 2.75E-01 -4.65E+01
PENRM MJ 5.31E-01 0 -2.9E-01 0 0 0 -1.81E-01 0
PENRT MJ 1.21E+02 9.89E+00 4.76E-02 0 2.33E-01 6.99E-02 9.47E-02 -4.65E+01
SM kg 3.45E-01 0 0 0 0 0 0 0
RSF MJ 0 0 0 0 0 0 0 0
NRSF MJ 0 0 0 0 0 0 0 0
FW m3 9.5E-02 1.05E-03 5.19E-05 0 2.47E-05 4.46E-05 2.17E-04 -3.7E-02
PERE = Use of renewable primary energy excluding renewable primary energy resources used as raw materials; PERM = Use of renewable primary
energy resources used as raw materials; PERT = Total use of renewable primary energy resources; PENRE = Use of non-renewable primary energy
excluding non-renewable primary energy resources used as raw materials; PENRM = Use of non-renewable primary energy resources used as raw
materials; PENRT = Total use of non-renewable primary energy resources; SM = Use of secondary material; RSF = Use of renewable secondary fuels;
NRSF = Use of non-renewable secondary fuels; FW = Use of net fresh water
RESULTS OF THE LCA – WASTE CATEGORIES AND OUTPUT FLOWS according to EN 15804+A2:
1 kg of window fittings
Parameter Unit A1-A3 A4 A5 C1 C2 C3 C4 D
HWD kg 9.5E-04 2.58E-05 2.15E-07 0 6.08E-07 2.46E-08 1.78E-07 2.9E-04
NHWD kg 3.63E+00 5.2E-01 3.19E-03 0 1.23E-02 2.61E-04 3.69E-01 -1.23E+00
RWD kg 6.24E-04 1.43E-04 6.17E-07 0 3.37E-06 9.32E-07 1.22E-06 -1.4E-04
CRU kg 0 0 0 0 0 0 0 0
MFR kg 6.66E-01 0 9.3E-02 0 0 4.9E-01 0 0
MER kg 0 0 0 0 0 0 0 0
6 Environmental Product Declaration - ARGE – The European Federation of Locks and Building Hardware Manufacturers - Window fittings
EEE MJ 6.46E-03 0 3.71E-02 0 0 0 7.66E-03 0
EET MJ 4.28E-02 0 2.45E-01 0 0 0 5.07E-02 0
HWD = Hazardous waste disposed; NHWD = Non-hazardous waste disposed; RWD = Radioactive waste disposed; CRU = Components for re-use;
MFR = Materials for recycling; MER = Materials for energy recovery; EEE = Exported electrical energy; EET = Exported thermal energy
RESULTS OF THE LCA – additional impact categories according to EN 15804+A2-optional:
1 kg of window fittings
Parameter Unit A1-A3 A4 A5 C1 C2 C3 C4 D
Disease
PM 8.64E-07 5.24E-08 3E-10 0 1.23E-09 4.5E-11 9.67E-10 -3.81E-07
incidence
IR kBq U235 eq 2.93E-01 4.29E-02 1.88E-04 0 1.01E-03 6.31E-04 4.03E-04 -6E-02
ETP-fw CTUe 5.14E+02 7.76E+00 4.49E-02 0 1.83E-01 3.49E-02 2.77E+01 -2.11E+02
HTP-c CTUh 3.66E-08 2.5E-10 3.37E-12 0 5.88E-12 9.32E-13 1.2E-11 -8.8E-09
HTP-nc CTUh 9.87E-07 7.84E-09 1.37E-10 0 1.85E-10 3.03E-11 1.34E-10 -2.88E-07
SQP SQP 6.41E+01 6.89E+00 3.03E-02 0 1.62E-01 1.07E-02 1.62E-01 -1.41E+01
PM = Potential incidence of disease due to PM emissions; IR = Potential Human exposure efficiency relative to U235; ETP-fw = Potential comparative
Toxic Unit for ecosystems; HTP-c = Potential comparative Toxic Unit for humans (cancerogenic); HTP-nc = Potential comparative Toxic Unit for humans
(not cancerogenic); SQP = Potential soil quality index
Disclaimer 1 – for the indicator 'Potential Human exposure efficiency relative to U235'. This impact category deals mainly with the
eventual impact of low-dose ionizing radiation on human health of the nuclear fuel cycle. It does not consider effects due to possible
nuclear accidents, occupational exposure or radioactive waste disposal in underground facilities. Potential ionizing radiation from the
soil, radon and from some construction materials is also not measured by this indicator.
Disclaimer 2 – for the indicators 'abiotic depletion potential for non-fossil resources', 'abiotic depletion potential for fossil resources',
'water (user) deprivation potential, deprivation-weighted water consumption', 'potential comparative toxic unit for ecosystems', 'potential
comparative toxic unit for humans – cancerogenic', 'Potential comparative toxic unit for humans - not cancerogenic', 'potential soil
quality index'. The results of this environmental impact indicator shall be used with care as the uncertainties on these results are high
as there is limited experience with the indicator.
6. LCA: Interpretation
Figure 1 illustrates the relative contributions of the different
modules along the life cycle of the declared products.
Figure 1: Environmental impacts of window fittings along Benefits and burdens beyond the system boundary (module D)
its life cycle are in the order of 20 % to 30 % of the impacts over the product
life cycle (modules A1-A3) and relate basically to the recycling
The largest part of environmental impacts is caused during of metals.
production (modules A1-A3); comparably small impacts are
caused during the transport of the product to the construction A total of 3 typical products (based on sales figures) have been
site (via the manufacturer of the product, which the window evaluated and the worst-case results are used in section 5 of
fitting has been integrated into). this EPD. In chapter 2.5, the tabulated range of relative weight
per material ensures that the variability of results stays within
All the other modules related to the product life cycle are not +/- 40% of the declared values (assessed for the indicators
significant. GWP, PENRT, and non-hazardous waste).
7 Environmental Product Declaration - ARGE – The European Federation of Locks and Building Hardware Manufacturers - Window fittings
7. Requisite evidence
No testing results are required by the PCR part B.
8. References
Product category rules of IBU 14044:2006.
IBU (2021) EN 13126
IBU (2021): General Instructions for the EPD Programme of the EN 13126, parts 1-19, various publication dates Building
Institut Bauen und Umwelt e.V. (General Instructions for the hardware – Requirements and test methods for windows and
IBU EPD Programme). Version 2.0, Institut Bauen und Umwelt, door height windows.
Berlin.
ISO 15686
IBU (2021) ISO 15686:1, -2, -7 and -8. Service life planning (various parts).
IBU (2021): PCR Part A: Calculation rules for the life cycle
assessment and requirements on the project report according ECHA candidate list
to EN 15804+A2. Version 1.3., Institut Bauen und Umwelt, Candidate List of substances of very high concern for
Berlin. Authorisation, published in accordance with Article 59(10) of the
REACH Regulation. European Chemicals Agency, Brussels.
IBU (2023)
IBU (2023): PCR Part B: Requirements on the EPD for building Ordinance on Biocide Products No. 528/2012
hardware products, Institut Bauen und Umwelt, Berlin. REGULATION (EU) No 528/2012 OF THE EUROPEAN
PARLIAMENT AND OF THE COUNCIL of 22 May 2012
Standards and legal documents concerning the making available on the market and use of
biocidal products.
EN 15804
EN 15804:2012+A2:2019+AC:2021, Sustainability of European List of Waste
construction works - Environmental product declarations - Core Commission Decision of 3 May 2000 replacing Decision
rules for the product category of construction products. 94/3/EC establishing a list of wastes pursuant to Article 1(a) of
Council Directive 75/442/EEC on waste and Council Decision
EN 17610 94/904/EC establishing a list of hazardous waste pursuant to
EN 17610:2022, Building hardware - Environmental product Article 1(4) of Council Directive 91/689/EEC on hazardous
declarations - Product category rules complementary to EN waste (notified under document number C(2000) 1147).
15804 for building hardware.
Additional references
ISO 14025
ISO 14025:2006-07, Environmental labels and declarations - BBSR 2017
Type III Environmental declarations - Principles and BBSR (2017): Nutzungsdauer von Bauteilen in
procedures. Lebenszyklusanalysen nach Bewertungssystem Nachhaltiges
Bauen (BNB). Version vom 24.10.2017, Bundesinstitut für Bau-,
ISO 14044 Stadt- und Raumforschung, Berlin.
EN ISO 14044:2006-07, Environmental management - Life
cycle assessment - Requirements and guidance (ISO ecoinvent v3.8
14044:2006); German and English versions EN ISO http://www.ecoinvent.org
8 Environmental Product Declaration - ARGE – The European Federation of Locks and Building Hardware Manufacturers - Window fittings
Publisher
Institut Bauen und Umwelt e.V. +49 (0)30 3087748- 0
Hegelplatz 1 info@ibu-epd.com
10117 Berlin www.ibu-epd.com
Germany
Programme holder
Institut Bauen und Umwelt e.V. +49 (0)30 3087748- 0
Hegelplatz 1 info@ibu-epd.com
10117 Berlin www.ibu-epd.com
Germany
Author of the Life Cycle Assessment
Dr. Frank Werner - Umwelt & Entwicklung + 41 (0)44 241 39 06
Kammelenbergstrasse 30 frank@frankwerner.ch
9011 St. Gallen http://www.frankwerner.ch/
Switzerland
Owner of the Declaration
ARGE – The European Federation of Locks and +49 (0)2051 9506 15
Building Hardware Manufacturers mail@arge.org
Offerstraße 12 www.arge.org
42551 Velbert
Germany
9 Environmental Product Declaration - ARGE – The European Federation of Locks and Building Hardware Manufacturers - Window fittings
