ENVIRONMENTAL PRODUCT DECLARATION
as per ISO 14025 and EN 15804+A2
Owner of the Declaration dormakaba International Holding GmbH
Publisher Institut Bauen und Umwelt e.V. (IBU)
Programme holder Institut Bauen und Umwelt e.V. (IBU)
Declaration number EPD-DOR-20210195-CBA2-EN
Issue date 07.10.2021
Valid to 06.10.2026
Extension module 90 30 / 90 31
dormakaba
www.ibu-epd.com | https://epd-online.com
General Information
dormakaba Extension module 90 30 / 90 31
Programme holder Owner of the declaration
IBU – Institut Bauen und Umwelt e.V. dormakaba International Holding GmbH
Hegelplatz 1 DORMA Platz 1
10117 Berlin 58256 Ennepetal
Germany Germany
Declaration number Declared product / declared unit
EPD-DOR-20210195-CBA2-EN 1 piece of the product: Extension module 90 30 / 90 31
This declaration is based on the product category rules: Scope:
Electronic and physical Access Control Systems, 01.08.2021 This EPD refers to a specific product manufactured by dormakaba. The
(PCR checked and approved by the SVR) production site is located in Villingen-Schwenningen (Germany).
The reference year is 2019.
Issue date The owner of the declaration shall be liable for the underlying information
and evidence; the IBU shall not be liable with respect to manufacturer
07.10.2021
information, life cycle assessment data and evidences.
The EPD was created according to the specifications of EN 15804+A2. In
Valid to
the following, the standard will be simplified as EN 15804.
06.10.2026
Verification
The standard EN 15804 serves as the core PCR
Independent verification of the declaration and data according to ISO
14025:2011
internally X externally
Dipl.-Ing. Hans Peters
(Chairman of Institut Bauen und Umwelt e.V.)
Florian Pronold Dr.-Ing. Wolfram Trinius,
(Managing Director Institut Bauen und Umwelt e.V.) (Independent verifier)
1 Environmental Product Declaration - dormakaba - Extension module 90 30 / 90 31
Product
Peripherals Interface
Product description/Product definition 90 30
Dormakaba extension modules allow a flexible set up of access • 8x relay output, switchover contact 30 V AC/DC; max. 2 A
control systems, providing the number of I/Os exactly required.
They connect to a dormakaba access manager 92 00 or to 90 31
remote readers 91 15 / 91 25. This offers not only 'made to • 8x line-monitored digital inputs, max. 5 V DC
measure' access control configurations but also the opportunity
to extend or adapt existing systems if requirements change Power supply
over time. For the placing on the market in the European • via proprietary bus from connected host device
Union/European Free Trade Association (EU/EFTA) (with the
exception of Switzerland) the following legal provisions apply: Installation
• Electromagnetic Compatibility Directive (EMC) • Top hat rails: TH35/(7.5/15)
• Low Voltage Directive (LVD) • Class of protection: IP20
• Restriction of Hazardous Substances (RoHS
• EN 50581:2012 The product is not harmonised in accordance with the
The CE-marking takes into account the proof of conformity with Construction Product Regulations (CPR) but in accordance with
the respective harmonized standards based on the legal other provisions for harmonisation of the EU. Compliance with
provisions above. For the application and use the respective the European Union Directive and technical specifications:
national provisions apply. • EN55032:2015
• EN55024:2016
Application
• EN62368-1:2014
Flexible access control The product is subject to CE marking according to the relevant
Activating door openers, external alarm systems or lift control harmonization legislation.
as well as monitoring sensors/door contacts as part of a In addition, the product also conforms to the following
comprehensive access control system. standards:
• Extended door control • UL 62368-1:2014
• Lift control • CAN/CSA-22.2 No. 62368-1:2014
• Alarm Management • UL 294 Security Level 1
• Window monitoring
Base materials/Ancillary materials
Technical Data
The major material compositions of the product are listed
The interface device 90 30 / 90 31 has the following technical below:
properties:
Name Value Unit
Name Value Unit
Electronics 46 %
Operating Temperature 0 - 40 °C
Paper 31 %
Operating Humidity 5 - 85 %
Plastics 23 %
Width Dimension 70 mm
Stainless steel <0,5 %
Height Dimension 99 mm
The product includes partial articles which contain substances
Depth Dimension 45 mm
listed in the Candidate List of REACH Regulation
Weight (without packaging) 0,144 kg
1907/2006/EC (date: 08.07.2021) exceeding 0.1 percentage by
Weight (with packaging) 0,192 kg mass in the alloy: No.
Power consumption "on mode" 5 W
Reference service life
Power consumption "idle mode" 2 W
The reference service life of the dormakaba interface device 90
Interface
30 / 90 31 is estimated to be 12 years. This number is based on
• proprietary in-line bus to host device
the support and service life and is not an estimated lifetime.
LCA: Calculation rules
Declared Unit Production - Module A1-A3
The declared unit is 1 piece of the product: Extension module The product stage includes:
90 30 / 90 31. — A1, raw material extraction, processing and mechanical
Declared unit treatments, processing of secondary material input (e.g.
recycling processes), — A2, transport to the manufacturer,
Name Value Unit
— A3, manufacturing and assembly including provision of all
Declared unit 1 pce.
materials, products and energy, as well as waste processing up
Conversion factor to 1 kg (kg per declared unit) 5.208 - to the end-of waste state.
Product weight including packaging 0,192 kg
Construction stage - Modules A4-A5
System boundary The construction process stage includes:
— A4, transport to the building site;
The type of EPD is: cradle to gate with options, modules C1–
— A5, installation into the building; including provision of all
C4, and module D (A1–A3 + C + D and additional modules: A4
materials, products and energy, as well as waste processing up
+ A5 + B6)
2 Environmental Product Declaration - dormakaba - Extension module 90 30 / 90 31
to the end-of-waste state or disposal of final residues during the includes:
construction process stage. — D, recycling potentials, expressed as net impacts and
benefits.
Use stage - Module B6
The use stage related to the operation of the building includes: Geographic Representativeness
— B6, operational energy use Land or region, in which the declared product system is
manufactured, used or handled at the end of the product´s
End-of-life stage– Modules C1-C4 and D lifespan: Germany
The end-of-life stage includes:
— C1, de-construction, demolition:
Comparability
— C2, transport to waste processing;
Basically, a comparison or an evaluation of EPD data is only
— C3, waste processing for reuse, recovery and/or recycling;
possible if all the data sets to be compared were created
— C4, disposal;
according to EN 15804 and the building context, respectively
including provision and all transport, provision of all materials,
the product-specific characteristics of performance, are taken
products and related energy and water use.
into account. Background database: GaBi, SP40.
Module D (Benefits and loads beyond the system boundary)
LCA: Scenarios and additional technical information
Operational energy use (B6) and Operational water use
Characteristic product properties of biogenic carbon
(B7)
Information on describing the biogenic Carbon Content at The use stage is declared for 12 years.
factory gate
Name Value Unit
Name ValueUnit
Energy consumption for 1 year 19,75 kWh
kg
Biogenic carbon content in product 0.01 on mode per day 2 h
C
idle mode per day 22 h
Biogenic carbon content in accompanying kg
0.02 on mode power 5 W
packaging C
idle mode 2 W
Note: 1 kg of biogenic carbon is equivalent to 44/12 kg of CO .
2 Days per year in use 365 days
End of life (C1-C4)
The following technical scenario information is required for the
C1: The product dismantling from the building is done manually
declared modules.
without environmental burden.
Transport to the building site (A4)
Name Value Unit
Name Value Unit Collected separately 0,14485 kg
Litres of fuel per 1 kg (truck) 0.00276 l/100km Recycling 0.089 kg
Transport distance (truck) 750 km Energy recovery 0.043 kg
Capacity utilisation (including empty runs) 51 % Landfilling 0.012 kg
Transport distance (ship) 1000 km Transportation to Waste Processing Site 50 km
Installation into the building (A5) Region for end of life: Global
Name Value Unit
Reuse, recovery and/or recycling potentials (D), relevant
Waste Packaging (paper) 0,05 kg
scenario information
Collection rate is 100%.
Reference service life
Name Value Unit
Life Span according to the manufacturer 12 a
3 Environmental Product Declaration - dormakaba - Extension module 90 30 / 90 31
LCA: Results
DESCRIPTION OF THE SYSTEM BOUNDARY (X = INCLUDED IN LCA; MND = MODULE OR INDICATOR NOT DECLARED; MNR
= MODULE NOT RELEVANT)
Benefits and
Construction loads beyond
Product stage Use stage End of life stage
process stage the system
boundaries
la ire ta m w a Ry lp p u s tro p s n a rT g n iru tc a fu n a M e h t m o rf tro p s n a rTe tis e h t o t e ta g y lb m e s s A e s U e c n a n e tn ia M ria p e R tn e m e c a lp e R tn e m h s ib ru fe R y g re n e la n o ita re p Oe s u re ta w la n o ita re p Oe s u n o itc u rts n o c -e Dn o itilo m e d tro p s n a rT g n is s e c o rp e ts a W la s o p s iD -e s u e R-y re v o c e R-g n ilc y c e Rla itn e to p
A1 A2 A3 A4 A5 B1 B2 B3 B4 B5 B6 B7 C1 C2 C3 C4 D
X X X X X MND MND MNR MNR MNR X MND X X X X X
RESULTS OF THE LCA - ENVIRONMENTAL IMPACT according to EN 15804+A2: 1 piece extension module 90 30 / 90 31
Parameter Unit A1-A3 A4 A5 B6 C1 C2 C3 C4 D
GWP-total kg CO 2 eq 2.38E+00 1.3E-02 6.7E-02 1.67E+02 0 4.34E-04 1.12E-01 1.89E-04 -8.8E-02
GWP-fossil kg CO 2 eq 2.39E+00 1.3E-02 2E-03 1.67E+02 0 4.15E-04 1.12E-01 1.87E-04 -8.8E-02
GWP-biogenic kg CO 2 eq -1.68E-02 5.6E-04 6.6E-02 2.82E-01 0 1.92E-05 2.6E-06 6.4E-07 -1.72E-04
GWP-luluc kg CO 2 eq 3.08E-03 3.01E-07 1.11E-06 1.63E-01 0 9.88E-09 6.31E-06 5.39E-07 -7.88E-05
ODP kg CFC11 eq 2.19E-10 1.34E-18 1.22E-17 2.26E-12 0 4.38E-20 5.63E-17 6.95E-19 -8.09E-16
AP mol H+ eq 1.81E-02 3.54E-05 1.89E-05 1.01E+00 0 4.15E-07 1.99E-05 1.34E-06 -4.95E-04
EP-freshwater kg P eq 1.24E-05 2.73E-09 2.38E-09 2.67E-04 0 8.88E-11 8.98E-09 3.22E-10 -1.02E-07
EP-marine kg N eq 3.04E-03 9.99E-06 6.82E-06 1.48E-01 0 1.32E-07 4.48E-06 3.46E-07 -6.44E-05
EP-terrestrial mol N eq 3.34E-02 1.1E-04 8.51E-05 1.6E+00 0 1.47E-06 9.05E-05 3.8E-06 -6.87E-04
kg NMVOC
POCP 9.11E-03 2.81E-05 1.81E-05 4.3E-01 0 3.74E-07 1.24E-05 1.05E-06 -1.98E-04
eq
ADPE kg Sb eq 9.7E-04 3.79E-10 1.92E-10 2.97E-05 0 1.25E-11 7.72E-10 1.68E-11 -2.32E-05
ADPF MJ 2.91E+01 1.79E-01 2.1E-02 2.4E+03 0 6E-03 5.2E-02 2E-03 -1.75E+00
m3 world eq
WDP 5E-01 2.49E-05 8E-03 2.95E+01 0 8.13E-07 1.1E-02 1.96E-05 -1.1E-02
deprived
GWP = Global warming potential; ODP = Depletion potential of the stratospheric ozone layer; AP = Acidification potential of land and water; EP =
Eutrophication potential; POCP = Formation potential of tropospheric ozone photochemical oxidants; ADPE = Abiotic depletion potential for non-fossil
resources; ADPF = Abiotic depletion potential for fossil resources; WDP = Water (user) deprivation potential)
RESULTS OF THE LCA - INDICATORS TO DESCRIBE RESOURCE USE according to EN 15804+A2: 1 piece extension module
90 30 / 90 31
Parameter Unit A1-A3 A4 A5 B6 C1 C2 C3 C4 D
PERE MJ 8.81E+00 5.66E-04 5.75E-01 7.96E+02 0 1.86E-05 1.62E-01 3.22E-04 -2.92E-01
PERM MJ 7.19E-01 0 -5.71E-01 0 0 0 -1.48E-01 0 0
PERT MJ 9.53E+00 5.66E-04 4E-03 7.96E+02 0 1.86E-05 1.3E-02 3.22E-04 -2.92E-01
PENRE MJ 2.72E+01 1.79E-01 2.1E-02 2.4E+03 0 6E-03 2.02E+00 2E-03 -1.75E+00
PENRM MJ 1.97E+00 0 0 0 0 0 -1.97E+00 0 0
PENRT MJ 2.91E+01 1.79E-01 2.1E-02 2.4E+03 0 6E-03 5.2E-02 2E-03 -1.75E+00
SM kg 0 0 0 0 0 0 0 0 0
RSF MJ 0 0 0 0 0 0 0 0 0
NRSF MJ 0 0 0 0 0 0 0 0 0
FW m3 1.3E-02 1.02E-06 1.97E-04 1.1E+00 0 3.33E-08 2.73E-04 6.2E-07 -3.5E-04
PERE = Use of renewable primary energy excluding renewable primary energy resources used as raw materials; PERM = Use of renewable primary
energy resources used as raw materials; PERT = Total use of renewable primary energy resources; PENRE = Use of non-renewable primary energy
excluding non-renewable primary energy resources used as raw materials; PENRM = Use of non-renewable primary energy resources used as raw
materials; PENRT = Total use of non-renewable primary energy resources; SM = Use of secondary material; RSF = Use of renewable secondary fuels;
NRSF = Use of non-renewable secondary fuels; FW = Use of net fresh water
RESULTS OF THE LCA – WASTE CATEGORIES AND OUTPUT FLOWS according to EN 15804+A2:
1 piece extension module 90 30 / 90 31
Parameter Unit A1-A3 A4 A5 B6 C1 C2 C3 C4 D
HWD kg 1.75E-06 1.74E-11 3.14E-11 1.27E-06 0 5.71E-13 1.97E-10 3.75E-11 -2.47E-09
NHWD kg 6E-02 1.83E-05 2E-03 1.39E+00 0 6.02E-07 1.2E-02 1.2E-02 2E-03
RWD kg 5.6E-04 1.93E-07 1.12E-06 2.68E-01 0 6.32E-09 1.92E-06 2.8E-08 -9.38E-05
CRU kg 0 0 0 0 0 0 0 0 0
MFR kg 0 0 0 0 0 0 4.3E-02 0 0
MER kg 0 0 0 0 0 0 0 0 0
EEE MJ 1.07E-01 0 1.02E-01 0 0 0 0 0 0
EET MJ 1.95E-01 0 1.85E-01 0 0 0 0 0 0
4 Environmental Product Declaration - dormakaba - Extension module 90 30 / 90 31
HWD = Hazardous waste disposed; NHWD = Non-hazardous waste disposed; RWD = Radioactive waste disposed; CRU = Components for re-use;
MFR = Materials for recycling; MER = Materials for energy recovery; EEE = Exported electrical energy; EET = Exported thermal energy
RESULTS OF THE LCA – additional impact categories according to EN 15804+A2-optional:
1 piece extension module 90 30 / 90 31
Parameter Unit A1-A3 A4 A5 B6 C1 C2 C3 C4 D
Disease
PM 1.61E-07 4.61E-10 1.05E-10 8.91E-06 0 2.18E-12 2.54E-10 1.66E-11 -4.09E-09
incidence
IR kBq U235 eq 5.1E-02 2.76E-05 1.73E-04 4.28E+01 0 9.03E-07 1.73E-04 2.88E-06 -1.5E-02
ETP-fw CTUe 1.14E+01 1.27E-01 1E-02 8.18E+02 0 4E-03 1.9E-02 1E-03 -4E-01
HTP-c CTUh 7.36E-10 2.39E-12 5.35E-13 2.6E-08 0 7.85E-14 1.68E-12 2.08E-13 -2.08E-11
HTP-nc CTUh 3.09E-08 1.03E-10 2.32E-11 1.06E-06 0 3.36E-12 1.7E-10 2.29E-11 -1.19E-09
SQP SQP 1.42E+01 4.61E-04 6E-03 5.67E+02 0 1.51E-05 1.5E-02 5.12E-04 -3.11E-01
PM = Potential incidence of disease due to PM emissions; IR = Potential Human exposure efficiency relative to U235; ETP-fw = Potential comparative
Toxic Unit for ecosystems; HTP-c = Potential comparative Toxic Unit for humans (cancerogenic); HTP-nc = Potential comparative Toxic Unit for humans
(not cancerogenic); SQP = Potential soil quality index
Disclaimer 1 – for the indicator IRP
This impact category deals mainly with the eventual impact of low dose ionizing radiation on human health of the nuclear fuel cycle. It
does not consider effects due to possible nuclear accidents, occupational exposure nor due to radioactive waste disposal in
underground facilities. Potential ionizing radiation from the soil, from radon and from some construction materials is also not measured
by this indicator.
Disclaimer 2 – for the indicators ADPE, ADPF, WDP, ETP-fw, HTP-c, HTP-nc, SQP
The results of this environmental impact indicator shall be used with care as the uncertainties on these results are high or as there is
limited experience with the indicator.
References
Standards requirements.
CAN/CSA-22.2 No. 62368-1 Electromagnetic Compatibility Directive
CAN/CSA-22.2 No. 62368-1:2014, Audio/video, information and Directive 2014/30/EU of the European Parliamant and of the
communication technologyequipment — Part 1: Safety Council of 26 February 2014 on the harmonisation of the laws
requirements. of the Member States relating to electromagnetic compatibility.
EN 15804+A2 ISO 14025
EN 15804:2019+A2 (in press), Sustainability of construction DIN EN ISO 14025:2011-10, Environmental labels and
works — Environmental Product Declarations — Core rules for declarations — Type III environmental declarations —
the product category of construction products. Principles and procedures.
EN 50581 Low Voltage Directive (LVD)
EN 50581:2012, Technical documentation for the assessment Directive 2014/35/EU of the European Parliament and of the
of electrical and electronic products with respect to the Council of 26 February 2014 on the harmonisation of the laws
restriction of hazardous substances. of the Member States relating to the making available on the
market of electrical equipment designed for use within certain
EN 55024 voltage limits.
EN 55024:2016, Information technology equipment - Immunity
characteristics - Limits and methods of measurement. Radio Equipment Directive (RED)
Directive 2014/53/EU of the European Parliament and of the
EN 55032 Council of 16 April 2014 on the harmonisation of the laws of the
EN 55032:2015, Electromagnetic compatibility of multimedia Member States relating to the making available on the market
equipment - Emission Requirements. of radio equipment and repealing Directive 1999/5/EC.
EN 60529
Degrees of protection provided by enclosures (IP 20). Registration, Evaluation, Authorisation and Restriction of
Chemicals (REACH)
EN 61000-3-2 Regulation (EC) No 1907/2006 of the European Parliament and
EN 61000-3-2:2013, Electromagnetic compatibility (EMC) - Part of the Council on the Registration, Evaluation, Authorisation
3-2: Limits - Limits for harmonic current emissions (equipment and Restriction of Chemicals (REACH).
input current ≤ 16 A per phase).
Restriction of Hazardous Substances (RoHS)
EN 61000-3-3 Directive on the restriction of the use of certain hazardous
EN 61000-3-3:2013, Electromagnetic compatibility (EMC) - Part substances in electrical and electronic equipment (RoHS),
3-3: Limits - Limitation of voltage changes, voltage fluctuations Directive (EU) No 2011/65.
and flicker in public low-voltage supply systems, for equipment
with rated current ≤ 16 A per phase and not subject to UL 294
conditional connection. UL 294:2013, Standard for Safety Access Control System Unit.
EN 62368-1+A11 UL 62368-1
EN 62368-1:2014+A11:2017, Audio/video, information and UL 62368-1:2014, Standard for Audio/video, information and
communication technology equipment - Part 1: Safety communication technology equipment - Part 1: Safety
5 Environmental Product Declaration - dormakaba - Extension module 90 30 / 90 31
requirements. documentation/).
Further References LCA-tool dormakaba
LCA tool, version 1.0.
IBU 2016
Institut Bauen und Umwelt e.V.: General Instructions for the Developed by Sphera Solutions GmbH.
EPD programme of Institut Bauen und Umwelt e.V. Version 2.0,
Berlin: Institut Bauen und Umwelt e.V., 2021. PCR Part A
PCR – Part A:
GaBi ts software Calculation Rules for the Life Cycle As-sessment and
Sphera Solutions GmbH Requirements on the Project Re-port according to EN
Gabi Software System and Database for Life Cycle Engineering 15804+A2:2019, Version 1.0, Institut Bauen und Umwelt e.V.,
1992-2020 Version 10.0.0.71 University of Stuttgart Leinfelden- www.ibu-epd.com.
Echterdingen
PCR Part B
GaBi ts documentation PCR – Part B: Requirements on the EPD for Building Hardware
GaBi life cycle inventory data documentation (https://www.gabi- product, version 1.3, Institut Bauen und Umwelt e.V., www.ibu-
software.com/support/gabi/gabi-database-2020-lci- epd.com, 2019.
6 Environmental Product Declaration - dormakaba - Extension module 90 30 / 90 31
Publisher
Institut Bauen und Umwelt e.V. +49 (0)30 3087748- 0
Hegelplatz 1 info@ibu-epd.com
10117 Berlin www.ibu-epd.com
Germany
Programme holder
Institut Bauen und Umwelt e.V. +49 (0)30 3087748- 0
Hegelplatz 1 info@ibu-epd.com
10117 Berlin www.ibu-epd.com
Germany
Author of the Life Cycle Assessment
Sphera Solutions GmbH +49 711 341817-0
Hauptstraße 111- 113 info@sphera.com
70771 Leinfelden-Echterdingen www.sphera.com
Germany
Owner of the Declaration
dormakaba International Holding GmbH +49 2333 793-0
DORMA Platz 1 info.de@dormakaba.com
58256 Ennepetal www.dormakaba.com
Germany
7 Environmental Product Declaration - dormakaba - Extension module 90 30 / 90 31
