ENVIRONMENTAL PRODUCT DECLARATION
as per ISO 14025 and EN 15804+A2
Owner of the Declaration Etex Building Performance International
Programme holder Institut Bauen und Umwelt e.V. (IBU)
Publisher Institut Bauen und Umwelt e.V. (IBU)
Declaration number EPD-ETE-20220189-ICA1-EN
Issue date 02.09.2022
Valid to 01.09.2027
PROMASTOP®-CC
Etex Germany Exteriors GmbH
www.ibu-epd.com | https://epd-online.com
Umwelt Produktdeklaration Name des Herstellers – Name des Produkts
1. General Information
Etex Germany Exteriors GmbH PROMASTOP®-CC
Programme holder Owner of the declaration
IBU – Institut Bauen und Umwelt e.V. Etex Building Performance International
Panoramastr. 1 500 Rue Marcel Demonque
10178 Berlin F-84915 Avignon
Germany France
Site of production
Etex Germany Exteriors GmbH
Im Breitspiel 20
69126 Heidelberg
Germany
Declaration number Declared product / declared unit
EPD-ETE-20220189-ICA1-EN The declared unit is 1 kg of PROMASTOP®-CC.
This declaration is based on the product Scope:
category rules: The life cycle assessment is based on production data
Coatings with organic binders, 01.2019 of PROMASTOP®-CC of the year 2020 at the
(PCR checked and approved by the SVR) production site Heidelberg, Germany.
Issue date The owner of the declaration shall be liable for the
02.09.2022 underlying information and evidence; the IBU shall not
be liable with respect to manufacturer information, life
cycle assessment data and evidences.
Valid to
The EPD was created according to the specifications
01.09.2027
of EN 15804+A2. In the following, the standard will be
simplified as EN 15804.
Verification
The standard EN 15804 serves as the core PCR
Independent verification of the declaration and data
according to ISO 14025:2010
Dipl. Ing. Hans Peters internally x externally
(chairman of Institut Bauen und Umwelt e.V.)
Dr. Alexander Röder Vito D'Incognito
(Managing Director Institut Bauen und Umwelt e.V.)) (Independent verifier)
2. Product
2.1 Product description/Product definition 2.2 Application
PROMASTOP®-CC is a water-based ‘hybrid’ fire PROMASTOP®-CC can be used as a coating for
stopping coating. It combines the positive qualities of coated batt system.
intumescent and ablative coatings. In the field of fire PROMASTOP®-CC is a fire stopping coating for
stopping penetrations, PROMASTOP®-CC provides services in walls and floors. It is designed for use with
reliable protection against the spread of smoke fire and single cables, cable bundles, combustible and non-
heat due to its foaming effect and simultaneous combustible pipes, fire dampers and also insulated
formation of a hard and solid char. ventilation systems to prevent the spread of smoke,
fire and heat.
For the placing of the product on the market in the
European Union/European Free Trade Association 2.3 Technical Data
(EU/EFTA) (with the exception of Switzerland) the
Regulation (EU) No. 305/2011 (CPR) applies. The
product needs a declaration of performance taking into Constructional data
consideration ETA 16/0523: 23.05.2017 and the CE-
marking. Name Value Unit
For the application and use the respective national Density 1500 kg/m3
provisions apply. Solids content 76 - 82 %
pH value 5.5 - 8.5 -log (a )
10 H+
VOC content according to ISO
<1 g/l
11890-2
2 Environmental Product Declaration Etex Germany Exteriors GmbH – PROMASTOP®-CC
Reaction to fire according to EN cleaning water is collected and professionally disposed
B-s1,d0 -
13501-1 by a disposal company.
Values are guidance values and do not reflect a The company and the manufacturing site have an
statistical evaluation or guaranteed value. environment, energy, health and safety management
system which is ISO 14001, ISO 50001 and ISO 45001
Performance data of the product in accordance with certified. The manufacturing plant adheres to the
the declaration of performance with respect to its German environmental and health and safety
essential characteristics according to ETA 16-0523, regulations.
23.05.2017.
2.8 Product processing/Installation
2.4 Delivery status PROMASTOP®-CC can be applied with a brush, roller
PROMASTOP®-CC is delivered in 5 kg or 12,5 kg or spatula.
plastic buckets.
2.9 Packaging
2.5 Base materials/Ancillary materials The coating is filled in plastic buckets made of
The main constituents of the product (in mass polypropylene (PP). The plastic buckets are packed on
percentages): pallets for shipping and are protected with polyethylene
Polymer emulsion (50 % in water) 25-50 % foil.
Aluminium hydroxide 25-50 %
Ammonium polyphosphate 10-20 %
Pigment TiO2 < 5 % 2.10 Condition of use
Graphite < 3 % PROMASTOP®-CC will form after drying, where water
Additives < 3 % is evaporating, a thin film and remains as such on the
Mineral fibre < 1 % substrate.
In-can preservatives < 0.225 %
Water 5 - 15 % 2.11 Environment and health during use
PROMASTOP®-CC is a fire stop coating with
1) This product contains substances listed in the extremely low emissions. Emission tests performed at
candidate list (date: 08.07.2021) exceeding 0.1 Eurofins confirm compliance with various national and
percentage by mass: no. international standards.
During the use phase, the product is considered to
2) This product contains other CMR substances in pose no health risk.
categories 1A or 1B which are not on the candidate
list, exceeding 0.1 percentage by mass: no 2.12 Reference service life
The intended use of PROMASTOP®-CC is assumed
3) Biocide products were added to this construction to be 10 years according to the ETA 16-0523,
product or it has been treated with biocide products 23.05.2017. An accelerated ageing test with the
(this then concerns a treated product as defined by the following fire test proved even a longer service life of
(EU) Ordinance on Biocide Products No. 528/2012): 30 to 33 years according to the Pavus test report.
yes. Above mentioned service life is related to ambient
In-can preservatives used are reaction mass of: 5- conditions, correct handling, installation and regular
chloro-2-methyl-4-isothiazolin-3-one [EC no. 247-500- inspection. Therefore the mentioned service life is not
7], and 2-methyl-2H -isothiazol-3-one [EC no. 220-239- a guarantee given by the manufacturer. It should help
6] (3:1) CAS 55965-84-9 (PT6), sodium pyrithione CAS to select an adequate product in accordance with the
3811-73-2 (PT6) and 1,2-benzisothiazol-3(2H)- building life- time.
one CAS 2634-33-5 (PT6).
2.6 Manufacture 2.13 Extraordinary effects
PROMASTOP®-CC is manufactured in a fully
automatic vacuum dissolver. The raw materials are Fire
dosed manually. PROMASTOP®-CC has the reaction to fire class B-
The raw materials undergo an incoming inspection by s1,d0 according to EN13501-1. In the event of a fire,
the quality laboratory before use. The produced batch due to the high temperatures, the coating forms a char
also goes through quality control and specific quality and delays the spread of fire. Once exposed to high
features are checked. External monitoring temperatures the coating has to be replaced.
for PROMASTOP®-CC takes place only with UL
marking.
The quality management system of the company and Fire protection
the production facility are certified according to Name Value
ISO9001. Building material class B
Burning droplets s1
2.7 Environment and health during Smoke gas development d0
manufacturing
Promat commits to a clean, healthy and safe working Water
environment for every person working in and for the PROMASTOP®-CC has the use category X. Therefore
company. the coating itself can be exposed to weathering. In
The raw materials are stored safely so that they cannot case of any extraordinary and longer exposure to
get into the surroundings/environment. There are water, the product would probably detach from the
adequately dimensioned extraction systems. Protective substrate. As the product is only used in low quantities
work clothing is made available to the employees. The in the building, it is expected that even following the
3 Environmental Product Declaration Etex Germany Exteriors GmbH – PROMASTOP®-CC
unforeseeable influence of water, the product would
not contribute to environmental damage. 2.15 Disposal
PROMASTOP®-CC must be disposed in a safe
Mechanical destruction manner in accordance with local/national regulations.
To ensure correct functionality repair works should be The waste code in accordance with the European List
done in accordance with the appropriate installation of Waste is 08 01 11* - waste paint and varnish
guidelines and in accordance with ETA 16-0523. No containing organic solvents or other dangerous
environmental impact is known related to mechanical substances.
destruction.
2.16 Further information
2.14 Re-use phase Further information is available on the following web
PROMASTOP®-CC could be used for energy recovery site :
in incineration plants, due to its organic substances in https://www.promat.com
the formulation.
3. LCA: Calculation rules
3.1 Declared Unit the product systems for the reference year
This declaration refers to the declared unit of 1 kg of 2020, temporal representativeness is good.
PROMASTOP®-CC. The density of PROMASTOP®-
 All primary and secondary data are collected
CC is 1500 kg/m³.
specific to the countries/regions under study.
Where country/region specific data are
Declared unit
Name Value Unit unavailable, proxy data are used. The overall
Gross density (mean value) 1500 kg/m3 geographical representativeness is
Declared unit 1 kg considered to be good.
 All primary and secondary data are modelled
to be specific to the technologies or
technology mixes under study. Where
3.2 System boundary
technology-specific data are unavailable,
The type of EPD is cradle to grave. The environmental
product declaration relates to the production stage proxy data are used. The overall
(module A1: provision of raw materials; A2: transport; technological representativeness is
A3: manufacture) and the construction process stage considered to be good.
(module A4: transport to the construction site and
 Primary data are collected by the client using
module A5: installation losses as well as the treatment
a specifically adapted spreadsheet. Sphera
of packaging material). The modules B1 to B7 are
supported the data collection by preparing a
declared with no impacts during the use stage. The
end-of-life stage is also considered (C1: dismantling, specific questionnaire and virtual or onsite
C2: transport to a disposal site, C3: no impacts from support.
waste processing and C4: disposal). The credits
outside the system boundary are taken into account in
Overall, the data quality can be described as good.
module D.
The primary data collection has been done thoroughly;
all relevant flows are considered.
3.3 Estimates and assumptions
3.7 Period under review
No major estimates or assumptions had to be made to
The period under review for the collection of production
the information provided in this EPD.
data is the year 2020.
3.4 Cut-off criteria
3.8 Allocation
No cut-off criteria are applied in this study. All reported
The production process does not deliver any co-
data were incorporated and modelled using the best
products. The applied software model does not contain
available LCI data.
any allocation.
3.5 Background data
The overall production of Etex Germany Exteriors
The background data has been taken from the latest
GmbH comprises further products besides the product
available GaBi database CUP 2021.2. The
considered in this study. Data for thermal and electrical
requirements for data quality and background data
energy refer to the declared product. During data
correspond to the specifications of the PCR Part A.
collection, the allocation is done via volume produced
per machine.
3.6 Data quality
The requirements on the data quality and the
3.9 Comparability
background data correspond to the provisions in EN
Basically, a comparison or an evaluation of EPD data
15804 and the IBU PCR part A (IBU 2020)
is only possible if all the data sets to be compared
respectively:
were created according to EN 15804 and the building
 All primary data are collected for the year
context, respectively the product-specific
2020. All secondary data come from the GaBi characteristics of performance, are taken into account.
databases and are representative of the years
2017-2020. As the study intended to compare
4 Environmental Product Declaration Etex Germany Exteriors GmbH – PROMASTOP®-CC
The used background database has to be mentioned Background dataset : GaBi ts software, CUP 2021.2.
4. LCA: Scenarios and additional technical information
Characteristic product properties waste
Information on biogenic Carbon Landfilling 1 kg
Biogenic carbon is only present in packaging (wooden
pallets). Reuse, recovery and/or recycling potentials (D),
Assumed water content in wooden pallet (packaging): relevant scenario information
18 %
The biogenic carbon content of the packaging is: For the thermal and electrical energy generated in
0,0597 kg pallet/declared unit * 0.82 * 0.5 kg C / kg Module A5 due to thermal treatment of packaging,
pallet (abs. dry) = 0.025 kg C/declared unit avoided burdens have been calculated by the inversion
of electricity grid mix and thermal energy from natural
Information on describing the biogenic Carbon gas, using European datasets.
Content at factory gate Metals from packaging (bucket handle) are assumed to
Name Value Unit reach the end of waste status directly at construction
Biogenic Carbon Content in site. The treatment and credits for avoided primary
0.025 kg C
accompanying packaging production (for the net scrap amount only) are grouped
to module D.
The following technical scenario information is required
for the declared modules.
Transport to the building site (A4)
Module A4 considers a 700 km truck transport from the
manufacturing plant in Heidelberg to an average
European customer site.
Name Value Unit
Transport distance 700 km
Capacity utilisation (including
61 %
empty runs)
Installation into the building (A5)
The installation of PROMASTOP-CC is done manually
and no energy is required. Installation losses have
been accounted for in module A5. Paint losses have
been considered as 2%.
The packaging material treatment and disposal are
also considered in module A5.
Name Value Unit
Electricity consumption 0 kWh
Material loss 0.02 kg
Output substances following
waste treatment on site 0.0977 kg
(packaging material)
End of life (C1-C4)
The end-of-life scenarios are as follows:
C1 – The deconstruction of the PROMASTOP-CC
coating is assumed to take place at the demolition of
the walls and the substrates onto which it is applied. In
this case, the environmental impact is assumed to be
very low. Therefore, no environmental loads for the
dismantling of this product is considered.
C2 – Transport to treatment/disposal site: Average
transport distance from the demolition site to waste
treatment is assumed as 50 km to landfill.
C4 – Disposal: The PROMASTOP-CC coatings are
100 % landfilled.
Name Value Unit
Collected as mixed construction 1 kg
5 Environmental Product Declaration Etex Germany Exteriors GmbH – PROMASTOP®-CC
5. LCA: Results
Disclaimer EP-freshwater:
This indicator has been calculated as “kg P eq” as required in the characterisation model (EUTREND model,
Struijs et al., 2009b, as implemented in ReCiPe; http://eplca.jrc.ec.europa.eu/LCDN/developerEF.xhtml).
DESCRIPTION OF THE SYSTEM BOUNDARY (X = INCLUDED IN LCA; ND = MODULE OR INDICATOR NOT
DECLARED; MNR = MODULE NOT RELEVANT)
BENEFITS AND
CONSTRUCTI LOADS
PRODUCT STAGE ON PROCESS USE STAGE END OF LIFE STAGE BEYOND THE
STAGE SYSTEM
BOUNDARIES
6 Environmental Product Declaration Etex Germany Exteriors GmbH – PROMASTOP®-CC
lairetam
waR
ylppus tropsnarT
gnirutcafunaM
eht
morf
tropsnarT
etis
eht
ot
etag
ylbmessA esU
ecnanetniaM
riapeR
tnemecalpeR tnemhsibrufeR
ygrene
lanoitarepO esu
retaw
lanoitarepO esu
noitcurtsnoc-eD
noitilomed tropsnarT
gnissecorp
etsaW
lasopsiD -esueR -yrevoceR -gnilcyceR laitnetop
A1 A2 A3 A4 A5 B1 B2 B3 B4 B5 B6 B7 C1 C2 C3 C4 D
X X X X X X X X X X X X X X X X X
RESULTS OF THE LCA - ENVIRONMENTAL IMPACT according to EN 15804+A2: 1 kg of PROMASTOP-CC
Core Indicator Unit A1-A3 A4 A5 B1 B2 B3 B4 B5 B6 B7 C1 C2 C3 C4 D
2.11E+ 0.00E+ 0.00E+ 0.00E+ 0.00E+ 0.00E+ 0.00E+ 0.00E+ 0.00E+ 0.00E+ -9.08E-
GWP-total [kg CO2-Eq.]
0
6.41E-22.61E-1
0 0 0 0 0 0 0 0
4.20E-3
0
1.51E-2
2
2.19E+ 0.00E+ 0.00E+ 0.00E+ 0.00E+ 0.00E+ 0.00E+ 0.00E+ 0.00E+ 0.00E+ -9.03E-
GWP-fossil [kg CO2-Eq.]
0
6.36E-21.70E-1
0 0 0 0 0 0 0 0
4.14E-3
0
1.51E-2
2
-7.72E- 0.00E+ 0.00E+ 0.00E+ 0.00E+ 0.00E+ 0.00E+ 0.00E+ 0.00E+ 0.00E+ 0.00E+ 0.00E+ -4.53E-
GWP-biogenic [kg CO2-Eq.]
2 0
9.04E-2
0 0 0 0 0 0 0 0
2.94E-5
0 0 4
0.00E+ 0.00E+ 0.00E+ 0.00E+ 0.00E+ 0.00E+ 0.00E+ 0.00E+ 0.00E+ -6.28E-
GWP-luluc [kg CO2-Eq.] 1.70E-35.22E-45.84E-5
0 0 0 0 0 0 0 0
3.40E-5
0
4.45E-5
5
1.41E- 8.15E- 3.76E- 0.00E+ 0.00E+ 0.00E+ 0.00E+ 0.00E+ 0.00E+ 0.00E+ 0.00E+ 5.30E- 0.00E+ 5.94E- -1.04E-
ODP [kg CFC11-Eq.]
14 18 16 0 0 0 0 0 0 0 0 19 0 17 15
0.00E+ 0.00E+ 0.00E+ 0.00E+ 0.00E+ 0.00E+ 0.00E+ 0.00E+ 0.00E+ -1.18E-
AP [mol H+-Eq.] 8.78E-32.19E-42.21E-4 1.42E-5 1.08E-4
0 0 0 0 0 0 0 0 0 4
0.00E+ 0.00E+ 0.00E+ 0.00E+ 0.00E+ 0.00E+ 0.00E+ 0.00E+ 0.00E+ -1.19E-
EP-freshwater [kg PO4-Eq.] 1.10E-51.89E-72.75E-7
0 0 0 0 0 0 0 0
1.23E-8
0
2.55E-8
7
0.00E+ 0.00E+ 0.00E+ 0.00E+ 0.00E+ 0.00E+ 0.00E+ 0.00E+ 0.00E+ -3.36E-
EP-marine [kg N-Eq.] 1.74E-31.02E-44.95E-5 6.62E-6 2.80E-5
0 0 0 0 0 0 0 0 0 5
0.00E+ 0.00E+ 0.00E+ 0.00E+ 0.00E+ 0.00E+ 0.00E+ 0.00E+ 0.00E+ -3.60E-
EP-terrestrial [mol N-Eq.] 1.77E-21.13E-35.62E-4 7.38E-5 3.07E-4
0 0 0 0 0 0 0 0 0 4
0.00E+ 0.00E+ 0.00E+ 0.00E+ 0.00E+ 0.00E+ 0.00E+ 0.00E+ 0.00E+ -9.43E-
POCP [kg NMVOC-Eq.]5.15E-31.97E-41.42E-4 1.28E-5 8.47E-5
0 0 0 0 0 0 0 0 0 5
0.00E+ 0.00E+ 0.00E+ 0.00E+ 0.00E+ 0.00E+ 0.00E+ 0.00E+ 3.16E- 0.00E+ -1.51E-
ADPE [kg Sb-Eq.] 4.25E-64.85E-98.73E-8 1.43E-9
0 0 0 0 0 0 0 0 10 0 8
-
4.52E+ 1.21E+ 0.00E+ 0.00E+ 0.00E+ 0.00E+ 0.00E+ 0.00E+ 0.00E+ 0.00E+ 0.00E+
ADPF [MJ] 8.49E-1 5.52E-2 2.01E-11.57E+
1 0 0 0 0 0 0 0 0 0 0
0
[m³ world-Eq 0.00E+ 0.00E+ 0.00E+ 0.00E+ 0.00E+ 0.00E+ 0.00E+ 0.00E+ 0.00E+ -6.97E-
WDP 2.69E-15.54E-42.52E-2 3.60E-5 1.62E-3
deprived] 0 0 0 0 0 0 0 0 0 3
GWP = Global warming potential; ODP = Depletion potential of the stratospheric ozone layer; AP = Acidification potential of land and water; EP =
Caption Eutrophication potential; POCP = Formation potential of tropospheric ozone photochemical oxidants; ADPE = Abiotic depletion potential for non-
fossil resources; ADPF = Abiotic depletion potential for fossil resources; WDP = Water (user) deprivation potential
RESULTS OF THE LCA - INDICATORS TO DESCRIBE RESOURCE USE according to EN 15804+A2: 1 kg of
PROMASTOP-CC
Indicator Unit A1-A3 A4 A5 B1 B2 B3 B4 B5 B6 B7 C1 C2 C3 C4 D
PERE [MJ] 7.64E+0 4.74E-2 1.07E+00.00E+00.00E+00.00E+00.00E+00.00E+00.00E+00.00E+00.00E+0 3.08E-3 0.00E+0 2.71E-2-3.57E-1
PERM [MJ] 8.80E-1 0.00E+0-8.80E-10.00E+00.00E+00.00E+00.00E+00.00E+00.00E+00.00E+00.00E+00.00E+00.00E+00.00E+00.00E+0
PERT [MJ] 8.52E+0 4.74E-2 1.92E-1 0.00E+00.00E+00.00E+00.00E+00.00E+00.00E+00.00E+00.00E+0 3.08E-3 0.00E+0 2.71E-2-3.57E-1
PENRE [MJ] 3.83E+1 8.50E-1 1.33E+00.00E+00.00E+00.00E+00.00E+00.00E+00.00E+00.00E+00.00E+0 5.53E-2 0.00E+07.12E+0-1.57E+0
PENRM [MJ] 7.03E+00.00E+0-1.10E-10.00E+00.00E+00.00E+00.00E+00.00E+00.00E+00.00E+00.00E+00.00E+00.00E+0-6.92E+00.00E+0
PENRT [MJ] 4.53E+1 8.50E-1 1.22E+00.00E+00.00E+00.00E+00.00E+00.00E+00.00E+00.00E+00.00E+0 5.53E-2 0.00E+0 2.01E-1-1.57E+0
SM [kg] 0.00E+00.00E+00.00E+00.00E+00.00E+00.00E+00.00E+00.00E+00.00E+00.00E+00.00E+00.00E+00.00E+00.00E+00.00E+0
RSF [MJ] 0.00E+00.00E+00.00E+00.00E+00.00E+00.00E+00.00E+00.00E+00.00E+00.00E+00.00E+00.00E+00.00E+00.00E+00.00E+0
NRSF [MJ] 0.00E+00.00E+00.00E+00.00E+00.00E+00.00E+00.00E+00.00E+00.00E+00.00E+00.00E+00.00E+00.00E+00.00E+00.00E+0
FW [m³] 9.74E-3 5.42E-5 7.39E-4 0.00E+00.00E+00.00E+00.00E+00.00E+00.00E+00.00E+00.00E+0 3.53E-6 0.00E+0 4.94E-5-3.49E-4
PERE = Use of renewable primary energy excluding renewable primary energy resources used as raw materials; PERM = Use of
renewable primary energy resources used as raw materials; PERT = Total use of renewable primary energy resources; PENRE = Use of
non-renewable primary energy excluding non-renewable primary energy resources used as raw materials; PENRM = Use of non-
Caption
renewable primary energy resources used as raw materials; PENRT = Total use of non-renewable primary energy resources; SM = Use
of secondary material; RSF = Use of renewable secondary fuels; NRSF = Use of non-renewable secondary fuels; FW = Use of net fresh
water
RESULTS OF THE LCA – WASTE CATEGORIES AND OUTPUT FLOWS according to EN 15804+A2:
1 kg of PROMASTOP-CC
Indicator Unit A1-A3 A4 A5 B1 B2 B3 B4 B5 B6 B7 C1 C2 C3 C4 D
-3.53E-
HWD [kg] 1.88E-84.28E-114.40E-100.00E+00.00E+00.00E+00.00E+00.00E+00.00E+00.00E+00.00E+02.79E-120.00E+02.14E-11
10
NHWD [kg] 1.12E+0 1.26E-4 4.37E-2 0.00E+00.00E+00.00E+00.00E+00.00E+00.00E+00.00E+00.00E+0 8.22E-6 0.00E+01.00E+0-7.39E-4
RWD [kg] 8.06E-4 1.03E-6 1.62E-5 0.00E+00.00E+00.00E+00.00E+00.00E+00.00E+00.00E+00.00E+0 6.69E-8 0.00E+0 2.07E-6-1.15E-4
CRU [kg] 0.00E+00.00E+00.00E+00.00E+00.00E+00.00E+00.00E+00.00E+00.00E+00.00E+00.00E+00.00E+00.00E+00.00E+00.00E+0
MFR [kg] 0.00E+00.00E+0 2.55E-3 0.00E+00.00E+00.00E+00.00E+00.00E+00.00E+00.00E+00.00E+00.00E+00.00E+00.00E+00.00E+0
MER [kg] 0.00E+00.00E+00.00E+00.00E+00.00E+00.00E+00.00E+00.00E+00.00E+00.00E+00.00E+00.00E+00.00E+00.00E+00.00E+0
EEE [MJ] 0.00E+00.00E+0 4.00E-1 0.00E+00.00E+00.00E+00.00E+00.00E+00.00E+00.00E+00.00E+00.00E+00.00E+00.00E+00.00E+0
EET [MJ] 0.00E+00.00E+0 7.14E-1 0.00E+00.00E+00.00E+00.00E+00.00E+00.00E+00.00E+00.00E+00.00E+00.00E+00.00E+00.00E+0
HWD = Hazardous waste disposed; NHWD = Non-hazardous waste disposed; RWD = Radioactive waste disposed; CRU = Components
Caption for re-use; MFR = Materials for recycling; MER = Materials for energy recovery; EEE = Exported electrical energy; EET = Exported
thermal energy
RESULTS OF THE LCA – additional impact categories according to EN 15804+A2-optional:
1 kg of PROMASTOP-CC
Indicator Unit A1-A3 A4 A5 B1 B2 B3 B4 B5 B6 B7 C1 C2 C3 C4 D
[Disease 7.81E-
PM 9.64E-8 1.20E-9 2.22E-90.00E+00.00E+00.00E+00.00E+00.00E+00.00E+00.00E+00.00E+0 0.00E+01.34E-9-1.02E-9
Incidence] 11
[kBq U235-
IRP 9.70E-2 1.47E-4 1.66E-30.00E+00.00E+00.00E+00.00E+00.00E+00.00E+00.00E+00.00E+09.58E-60.00E+02.13E-4-1.88E-2
Eq.]
ETP-fw [CTUe] 2.08E+16.13E-1 5.85E-10.00E+00.00E+00.00E+00.00E+00.00E+00.00E+00.00E+00.00E+03.99E-20.00E+01.14E-1-3.30E-1
1.24E- 7.61E- 8.05E- 1.69E- -1.50E-
HTP-c [CTUh] 3.50E-9 0.00E+00.00E+00.00E+00.00E+00.00E+00.00E+00.00E+00.00E+0 0.00E+0
11 11 13 11 11
7.41E- 4.82E- -5.89E-
HTP-nc [CTUh] 3.76E-7 7.87E-90.00E+00.00E+00.00E+00.00E+00.00E+00.00E+00.00E+00.00E+0 0.00E+01.86E-9
10 11 10
SQP [-] 3.66E+12.91E-1 7.64E-10.00E+00.00E+00.00E+00.00E+00.00E+00.00E+00.00E+00.00E+01.90E-20.00E+04.24E-2-2.44E-1
PM = Potential incidence of disease due to PM emissions; IR = Potential Human exposure efficiency relative to U235; ETP-fw = Potential
Caption comparative Toxic Unit for ecosystems; HTP-c = Potential comparative Toxic Unit for humans (cancerogenic); HTP-nc = Potential
comparative Toxic Unit for humans (not cancerogenic); SQP = Potential soil quality index
Disclaimer 1 – for the indicator “Potential Human exposure efficiency relative to U235”.
This impact category deals mainly with the eventual impact of low-dose ionizing radiation on human health of the
nuclear fuel cycle. It does not consider effects due to possible nuclear accidents, occupational exposure or
radioactive waste disposal in underground facilities. Potential ionizing radiation from the soil, radon and from
some construction materials is also not measured by this indicator.
Disclaimer 2 – for the indicators “abiotic depletion potential for non-fossil resources”, “abiotic depletion potential
for fossil resources”, “water (user) deprivation potential, deprivation-weighted water consumption”, “potential
comparative toxic unit for ecosystems”, “potential comparative toxic unit for humans – cancerogenic”, “Potential
comparative toxic unit for humans - not cancerogenic”, “potential soil quality index”. The results of this
environmental impact indicator shall be used with care as the uncertainties on these results are high as there is
limited experience with the indicator.
6. LCA: Interpretation
The interpretation is based on the assumptions and The following figure shows the results of the individual
limitations described in this background report, both modules as an example for the global warming
with regard to the methods and the data. A dominance potential.
analysis is used for interpretation.
7 Environmental Product Declaration Etex Germany Exteriors GmbH – PROMASTOP®-CC
during plant growth in connection with
It is visible that the manufacturing phase dominates the packaging (wooden pallet). The packaging
product system. In addition, the packaging treatment in
makes moderate contributions in all other
module A5 has relevant environmental impacts.
impact categories.
 Titanium dioxide has a significant impact on
Interpretation of results for the environmental
indicators according to ISO 14044: the resource use of minerals and metals
 The resin has a significant influence (>50 %) indicator (ADPm).
on the ADPF and water use indicators and a  The ammonium polyphosphate has a relevant
relevant influence (entre 25 % et 50 %) on the influence on the AP indicator.
GWP, ODP, EP and POCP indicators.
 The biogenic global warming potential shows
the absorption of atmospheric carbon dioxide
7. Requisite evidence
AgBB overview of results (28 days [µg/m³])
7.1 VOC emissions Name Value Unit
VOC emission measurements confirmed compliance TVOC (C6 - C16) 44 μg/m3
with the AgBB/ABG requirements. Sum SVOC (C16 - C22) 24 μg/m3
R (dimensionless) 0.19 -
VOC without NIK <5 μg/m3
Carcinogenic Substances <1 μg/m3
Formaldehyde <3 µg/m³
Date: 11 April 2019
Measuring agency: Eurofins Product Testing A/S,
Galten, Denmark
Report number: 392-2019-00089002_A_EN
8. References
Standards Declarations — Core rules for the product category of
construction products.
EN 13501-1
EN 13501-1:2007+A1:2009, Fire classification of ISO 9001
construction products and building elements - Part 1: UNI EN ISO 9001:2015 September 2015, Quality
Classification using data from reaction to fire tests. management systems - Requirements
EN 15804 ISO 11890-2
EN 15804:2012+A2:2019, Sustainability of ISO 11890-2:2013 Paints and varnishes —
construction works — Environmental Product
8 Environmental Product Declaration Etex Germany Exteriors GmbH – PROMASTOP®-CC
Determination of volatile organic compound (VOC) GaBi
content — Part 2: Gas-chromatographic method. GaBi Software System and Database for Life Cycle
Engineering, 1992-2021, Sphera Solutions GmbH,
ISO 14001 Leinfelden-Echterdingen, with acknowledgement of
UNI EN ISO 14001:2015, Environmental management LBP University of Stuttgart, program version GaBi 10;
systems - Requirements with guidance for use. database version 2021.1.
ISO 14025 GaBi documentation
DIN EN ISO 14025:2011-10, Environmental labels and GaBi dataset documentation for the software system
declarations — Type III environmental declarations — and databases, LBP, University of Stuttgart and
Principles and procedures. Sphera Solutions GmbH, Leinfelden-Echterdingen,
2021.
ISO 45001 (http://www.gabi-software.com/support/gabi/gabi-
ISO 45001:2018, Occupational health and safety database-2021-lci-documentation/)
management systems — Requirements with guidance
for use IBU 2021
Institut Bauen und Umwelt e.V.: General Programme
ISO 50001 Instructions for the Preparation of EPDs at the Institut
ISO 50001:2018, Energy management systems — Bauen und Umwelt e.V. Version 2.0, Berlin: Institut
Requirements with guidance for use Bauen und Umwelt e.V., 2021
Further References Ordinance on Biocide Products
Regulation (EU) No 528/2012 of the European
AgBB/AGB Parliament and of the Council of 22 May 2012
Ausschuss zur gesundheitlichen Bewertung von concerning the making available on the market and
Bauprodukten, AgBB. Anforderungen an bauliche use of biocidal products.
Anlagen bezüglich des Gesundheitsschutzes, AGB.
(eng. German Committee for health-related evaluation Pavus
of building products. Fire testing laboratory, Veselí nad Lužnicí, Czech
Republic.
Candidate list Report number 60193174, 2016.
Candidate List of substances of very high concern for
Authorisation, published on ECHA website, latest PCR Part A
version 08.07.2021. (https://echa.europa.eu/candidate- PCR Part A: Calculation rules for the Life Cycle
list-table) Assessment and Requirements on the Background
Report according to EN 15 804+A2:2019, Version 1.0,
CPR Institut Bauen und Umwelt e.V., 2020.
Construction Products Regulation, Regulation (EU) No
305/2011 of the European Parliament and of the PCR Part B
Council of 9 March 2011 laying down harmonized Product Category Rules for Building Products, Part B:
conditions for the marketing of construction products Requirements on the EPD for coatings with organic
and repealing Council Directive 89/106/ EEC Text with binders, version 1.7, 2019 www.bau-umwelt.de
EEA relevance.
REACH Regulation
European List of Waste Regulation (EU) No 1907/2006 of the European
2014/955/EU: Commission Decision of 18 December Parliament and of the Council of 18 December 2006
2014 amending Decision 2000/532/EC on the list of concerning the Registration, Evaluation, Authorisation
waste pursuant to Directive 2008/98/EC of the and Restriction of Chemicals (REACH), establishing a
European Parliament and of the Council. European Chemicals Agency, amending Directive
(http://data.europa.eu/eli/dec/2014/955/oj) 1999/45/EC and repealing Council Regulation (EEC)
No 793/93 and Commission
ETA 16/0523 Regulation (EC) No 1488/94 as well as Council
European technical approval of PROMASTOP®-CC. Directive 76/769/EEC and Commission Directives
91/155/EEC, 93/67/EEC, 93/105/EC and 2000/21/EC.
Eurofins Product Testing A/S
Eurofins Product Testing A/S, Smedeskovvej 38, 8464
Galten, Denmark. Report number: 392-2019-
00089002_A_EN
9 Environmental Product Declaration Etex Germany Exteriors GmbH – PROMASTOP®-CC
Publisher
Institut Bauen und Umwelt e.V. Tel +49 (0)30 3087748- 0
Panoramastr. 1 Fax +49 (0)30 3087748- 29
10178 Berlin Mail info@ibu-epd.com
Germany Web www.ibu-epd.com
Programme holder
Institut Bauen und Umwelt e.V. Tel +49 (0)30 - 3087748- 0
Panoramastr 1 Fax +49 (0)30 – 3087748 - 29
10178 Berlin Mail info@ibu-epd.com
Germany Web www.ibu-epd.com
Author of the Life Cycle
Assessment Tel +49 711 341817-0
Sphera Solutions GmbH Fax +49 711 341817-25
Hauptstraße 111- 113 Mail info@sphera.com
70771 Leinfelden-Echterdingen Web www.sphera.com
Germany
Owner of the Declaration
Etex Building Performance Tel +32 2 778 12 11
International Fax +32 2 778 12 12
Rue Marcel Demonque 500 Mail info@etexgroup.com
84915 Avignon Cedex 9 Web http://www.etexgroup.com
France
