ENVIRONMENTAL PRODUCT DECLARATION
as per ISO 14025 and EN 15804+A2
Owner of the Declaration Stiferite
Publisher Institut Bauen und Umwelt e.V. (IBU)
Programme holder Institut Bauen und Umwelt e.V. (IBU)
Declaration number EPD-STF-20220329-CBC2-EN
Issue date 16.02.2023
Valid to 15.02.2028
Stiferite PENDENZATO GT
Stiferite
www.ibu-epd.com | https://epd-online.com
General Information
Stiferite Stiferite PENDENZATO GT
Programme holder Owner of the declaration
IBU – Institut Bauen und Umwelt e.V. Stiferite
Hegelplatz 1 Viale Navigazione Interna 54
10117 Berlin 35129 Padova
Germany Italy
Declaration number Declared product / declared unit
EPD-STF-20220329-CBC2-EN Stiferite PENDENZATO GT is a composite panel made by a base side
EPS and a top side based on Stiferite GT, expanded rigid polyurethane
foam, covered on both sides by multi-layer facer, and produced by Stiferite.
The EPD applies to 1 m2 of 63 mm thick PUR sandwich board and 30 mm
thick EPS slope board, i.e. 0.093 m3, with an average density between
foam and facing of 32.4 kg/m3.
This declaration is based on the product category rules: Scope:
Insulating materials made of foam plastics, 01.08.2021 Stiferite produces StiferitePENDENZATO GT which is a high performance
(PCR checked and approved by the SVR) composite insulation board manufactured from a top side a closed cell
expanded rigid polyurethane foam, covered on both sides by multi-layer
facer, and a bottom side an EPS insulation panel with a slope shape. The
Issue date data have been provided by the only Stiferite factory that is located in
Padova (Italy) for the year 2021 and sold worldwide.
16.02.2023
The owner of the declaration shall be liable for the underlying information
and evidence; the IBU shall not be liable with respect to manufacturer
information, life cycle assessment data and evidences.
Valid to
15.02.2028 The EPD was created according to the specifications of EN 15804+A2. In
the following, the standard will be simplified as EN 15804.
Verification
The standard EN 15804 serves as the core PCR
Independent verification of the declaration and data according to ISO
14025:2011
internally X externally
Dipl.-Ing. Hans Peters
(Chairman of Institut Bauen und Umwelt e.V.)
Dipl.-Ing. Hans Peters Prof. Dr. Birgit Grahl,
(Managing Director Institut Bauen und Umwelt e.V.) (Independent verifier)
1 Environmental Product Declaration - Stiferite - Stiferite PENDENZATO GT
Product
EPS side EN 13163:2012+A2:2016. Thermal insulation
Product description/Product definition products for building- factory made expanded polystyrene
Stiferite's thermal insulation panels are mainly used in the (EPS) products - Specification and the CE-marking.. For the
building/construction sector and in industrial insulation. application and use the respective national provisions apply.
The panels are made of thermo-setting closed cells
polyurethane foam (PU) supplied with various types of flexible Base materials/Ancillary materials
facers on both sides of the panel. The nature/type of facer is a PU insulation panel: (about 65.2 % of the weight of the
function of the type of panel and its application. declared unit)
Expanded rigid polyurethane foam is distinguished by its
thermal insulation performance, mechanical resistance, Close cell Polyiso (PIR): rigid foam made from MDI (50-65 %),
workability, lightness, and durability. polyols (20-30 %), pentane (4-6 %) and additives (4-6 %).
The performance of Stiferite's panels is determined based on PU Facing (about 5.1 % of the weight of the declared unit):
the European norm EN13165:2012+A2:2016 Thermal multi-layer facer consisting of aliminium (10-20 %), kraft paper
insulation products for buildings - Factory-made rigid (60-70 %) and PE layer (10-20 %).
polyurethane foam (PU) products - Specification. EPS insulation panel: about 29.7 %
This EPD refers to Stiferite's PENDENZATO GT average thick
panel, , made of an insulation component in polyurethane foam The PU and EPS boards for insulation:
using blowing agent Pentane-based, covered on both sides by
• This product/article/at least one partial article contains
multi-layer facer, and on the bottom side of an insulation
substances listed in the candidate list (date: 17.01.2022)
component in EPS with a slope shape The panel is produced in
exceeding 0.1 percentage by mass: no
standard dimensions of as request by the customers and
straight finish borders. • This product/article/at least one partial article doesn't
Stiferite PENDENZATO GT panel is produced by a certified contain other carcinogenic, mutagenic, reprotoxic
company with systems:ISO 9001, ISO 45001, ISO 14001 in its (CMR) substances in categories 1A or 1B which are not
entire line of products. on the candidate list, exceeding 0.1 percentage by
mass: no
Application
• Biocide products were added to this construction
The Stiferite PENDENZATO GT panel is suitable for the product or it has been treated with biocide products (this
insulation of flat roofs under synthetic mantles in-view or then concerns a treated product as defined by the (EU)
weighted down and under bituminous mantles applied cold (not Ordinance on Biocide Products No.528/2012): no
torched). Additional declaration according to quoted law: The product is
compliant with all requirements indicated in chapter 2.5.7
Technical Data
'Isolanti termici ed acustici' of the n.256 D.L. of the 23th June
In this Life Cycle Assessment, a PU insulation board with the
2022 (CAM EDILIZIA)
following properties has been regarded:
• Any blowing agent with Ozone depletion potential >0 is
Constructional data
not used in production
Name Value Unit • Any substances of Very High Concern-SVHC in
Gross density 32.4 kg/m3 concentration of more than 0,1 %w are not used in
production (REACH n. 1907/2006). Any specific
Declared Average Thermal PU:0.022,
W/mK authorizations for use are eserved provided for by the
conductivity λD acc. to EN 13165 EPS:0,033
same Regulation for the substances included in Annex
Compressive strength at 10%
>150 kPa XIV and specifications restrictions set out in Annex XVII
deformation acc. to EN 826
of the Regulation.
Tensile strength perpendicular to the >30 kPa • Catalysts lead-based are not used in production
face acc. to EN 1607 • Flame retardants used in production (belonging to the
Water absorption by total immersion Vol.- Organophosphorus class) are not banned by any
<2
acc. to EN 12087 % national or European regulation
Water absorption by partial immersion • According to the raw materials declarations of suppliers,
< 0.1 kg/m²
acc. to EN 1609 the minimum amount of recycled raw materials based
on the EPS insulation weight is more than 15% and
Water vapour diffusion resistance PU:56, EPS:30- w
factor μ acc. to EN 12086 70 based on the PU insulation board (PU foam and facers)
weight is 3 % and the minimum amount of recycled
Euroclass reaction to fire acc. to EN w
E
11925 raw materials based on the PU insulation foam weight is
4 % in compliance with REMADE in Italy type 1
This provides a thermal resistance R = 4.7 m² k/W. w
certification (note: this information is not explicitly
considered in the LCA and not included in the EPD
Product according to the CPR based on a
tables that only refer to recycling content in the
hEN/:13165:2012+A2:2016 For the placing on the market of the
foreground system).
product in the European Union/European Free Trade
Association (EU/EFTA) (with the exception of Switzerland)
Reference service life
Regulation (EU) No.305/2011 (CPR) applies. The product
The durability of insulation panels is normally at least as long as
needs a Declaration of Performance taking into consideration
the lifetime of the building in which it is used. The experimental
for polyurethane side EN 13165:2012+A2:2016. Thermal
data show that the reference life is greater than 50 years.
insulation products for building- factory made rigid polyurethane
foam (PU) products - Specification and the CE-marking, and for
2 Environmental Product Declaration - Stiferite - Stiferite PENDENZATO GT
LCA: Calculation rules
thermal insulation board. The life cycle is split into the following
Declared Unit individual phases:
The declared unit is 1 m² with a thickness of 93 mm, e. g. 0.093 A1 - Raw material formulation
m³. A2 - Raw material transport
Corresponding conversion factors are listed in the table below. A3 - Production of the insulation board and packaging material
Declared unit A4 - Transport to the construction site
C1 - demolition and deconstruction
Name Value Unit
C2 - Transport to end of life
Declared unit 1 m2 C3 - End-of-Life: waste management (thermal recovery)
Gross density 32.4 kg/m3 C4 - End-of-Life: waste management (landfill)
Grammage 3.01 kg/m2 D - Benefits and loads beyond system boundary
Layer thickness 0.093 m Geographic Representativeness
Declared average thermal PU:0.022, Land or region, in which the declared product system is
W/mK
conductivity λD EPS:0.033 manufactured, used or handled at the end of the product´s
lifespan: Italy
This provides a thermal resistance R = 4.7 m² /W.
Comparability
System boundary Basically, a comparison or an evaluation of EPD data is only
possible if all the data sets to be compared were created
Type of the EPD: cradle to gate - with options
according to EN 15804 and the building context, respectively
This life cycle assessment for the production of the
the product-specific characteristics of performance, are taken
polyurethane insulation board considers the life cycle from the
into account. The background database used is GaBi 2022
supply of raw materials to the manufacturer´s gate (cradle-to-
database (v. 2022.1)
gate with options). It also includes the transport to the
construction site and the end-of-life stage of the used PU
LCA: Scenarios and additional technical information
Characteristic product properties of biogenic carbon
End of life (C1-C4)
Name Value Unit
Information on describing the biogenic Carbon Content at
Scenario No 1: Material Incineration 100 %
factory gate
Scenario No 2: Landfill 100 %
Name ValueUnit
kg C1 – Deconstruction and demolition (0.2 MJ/kg as electrical
Biogenic carbon content in product 43 C consumption assumed)
Biogenic carbon content in accompanying kg
0.003 C2 – Panel is transported from the building site to a treatment
packaging C
plant by truck and an average distance of 100 km is
considered.
C3/C4- Disposal scenarios used are divided into 2 sub-
Transport to the building site (A4) scenarios:
1) Incineration 100 % (C3/1)
Name ValueUnit
2) Landfilling 100 % (C4/2)
Truck with a capacity of 17.3 tons 59.6 km
Ferry with a capacity of 1200-10000 dwt payload
0 km Reuse, recovery and/or recycling potentials (D), relevant
capacity
scenario information
Ship with a capacity of 27500 dwt payload capacity
0 km D: Benefits and loads beyond system boundary are divided into
tons
2 sub-scenarios:
Plane with a capacity of 22 ton 0 km
Name Value Unit
Type and amount of packaging included in module A3 Scenario No 1: Material Incineration 100 %
Name Value Unit Scenario No 2: Landfill 100 %
Cardboard 0.00691 kg
EPS stock 0.00578 kg
EPS stock - glue 0.00041 kg
Paper labels 0.00014 kg
PE film 0.03869 kg
PP tape 0.00005 kg
PUR stucks 0 kg
SBR labels 0.00001 kg
TOTAL PACKAGING 0.05199 kg
3 Environmental Product Declaration - Stiferite - Stiferite PENDENZATO GT
LCA: Results
The tables below show the results of the LCA. Basic information on all declared modules provides chapter 4.
There are two scenarios for the end-of-life (C2, C4 and D) analyzed: Scenario 1 considers 100 % incineration, Scenario 2 considers
100 % landfill disposal.
For SM, RSF, NRSF, CRU indicators only the foreground system is considered.
DESCRIPTION OF THE SYSTEM BOUNDARY (X = INCLUDED IN LCA; ND = MODULE OR INDICATOR NOT DECLARED; MNR =
MODULE NOT RELEVANT)
Benefits and
Construction loads beyond
Product stage Use stage End-of-life stage
process stage the system
boundaries
la ire ta m w a Ry lp p u s tro p s n a rT g n iru tc a fu n a M e h t m o rf tro p s n a rTe tis e h t o t e ta g y lb m e s s A e s U e c n a n e tn ia M ria p e R tn e m e c a lp e R tn e m h s ib ru fe R y g re n e la n o ita re p Oe s u re ta w la n o ita re p Oe s u n o itc u rts n o c -e Dn o itilo m e d tro p s n a rT g n is s e c o rp e ts a W la s o p s iD -e s u e R-y re v o c e R-g n ilc y c e Rla itn e to p
A1 A2 A3 A4 A5 B1 B2 B3 B4 B5 B6 B7 C1 C2 C3 C4 D
X X X X MND MND MND MNR MNR MNR MND MND X X X X X
RESULTS OF THE LCA - ENVIRONMENTAL IMPACT according to EN 15804+A2: 1 m2 PENDENZATO GT
Parameter Unit A1-A3 A4 C1 C2 C3/1 C3/2 C4/1 C4/2 D/1 D/2
GWP-total kg CO 2 eq 1.07E+01 1.56E-02 6.87E-02 1.82E-02 7.37E+00 0 0 2.44E-01 -3.39E+00 0
GWP-fossil kg CO 2 eq 1.09E+01 1.54E-02 6.87E-02 1.8E-02 7.23E+00 0 0 1.02E-01 -3.38E+00 0
GWP-
biogenic kg CO 2 eq -2.1E-01 5.02E-05 4.05E-05 5.84E-05 1.38E-01 0 0 1.42E-01 -3.51E-03 0
GWP-luluc kg CO 2 eq 3.2E-03 1.04E-04 4.45E-06 1.21E-04 1.28E-05 0 0 8.97E-05 -1.67E-04 0
ODP kg CFC11 eq 1.24E-11 1.52E-15 6.78E-13 1.77E-15 4.74E-13 0 0 1.67E-13 -2.1E-11 0
AP mol H+ eq 1.56E-02 5.49E-05 1.01E-04 6.01E-05 3E-03 0 0 4.38E-04 -3.83E-03 0
EP-
kg P eq 2.36E-05 5.53E-08 3.08E-08 6.43E-08 1.29E-07 0 0 1.3E-05 -1.03E-06 0
freshwater
EP-marine kg N eq 4.51E-03 2.53E-05 2.76E-05 2.75E-05 1.39E-03 0 0 1.17E-04 -1.16E-03 0
EP-terrestrial mol N eq 4.67E-02 2.83E-04 2.95E-04 3.08E-04 1.65E-02 0 0 1.18E-03 -1.25E-02 0
kg NMVOC
POCP 3.79E-02 4.94E-05 7.79E-05 5.4E-05 3.59E-03 0 0 3.75E-04 -3.31E-03 0
eq
ADPE kg Sb eq 1.93E-06 1.56E-09 8.17E-09 1.81E-09 1.25E-08 0 0 8.04E-09 -3.12E-07 0
ADPF MJ 2.61E+02 2.03E-01 1.46E+00 2.36E-01 1.57E+00 0 0 1.41E+00 -6.53E+01 0
m3 world eq
WDP 1.63E+00 1.73E-04 5.13E-03 2.01E-04 6.88E-01 0 0 3.11E-03 -1.62E-01 0
deprived
GWP = Global warming potential; ODP = Depletion potential of the stratospheric ozone layer; AP = Acidification potential of land and water; EP =
Eutrophication potential; POCP = Formation potential of tropospheric ozone photochemical oxidants; ADPE = Abiotic depletion potential for non-fossil
resources; ADPF = Abiotic depletion potential for fossil resources; WDP = Water (user) deprivation potential)
RESULTS OF THE LCA - INDICATORS TO DESCRIBE RESOURCE USE according to EN 15804+A2: 1 m2 PENDENZATO GT
Parameter Unit A1-A3 A4 C1 C2 C3/1 C3/2 C4/1 C4/2 D/1 D/2
PERE MJ 1.29E+01 1.41E-02 2.1E-01 1.64E-02 1.98E+00 0 0 1.83E+00 -6.59E+00 0
PERM MJ 1.81E+00 ND ND ND -1.69E+00 0 0 -1.69E+00 ND 0
PERT MJ 1.47E+01 1.41E-02 2.1E-01 1.64E-02 2.91E-01 0 0 1.42E-01 -6.59E+00 0
PENRE MJ 1.69E+02 2.04E-01 1.46E+00 2.37E-01 9.13E+01 0 0 9.12E+01 -6.53E+01 0
PENRM MJ 9.19E+01 ND ND ND -8.98E+01 0 0 -8.98E+01 ND 0
PENRT MJ 2.61E+02 2.04E-01 1.46E+00 2.37E-01 1.57E+00 0 0 1.41E+00 -6.53E+01 0
SM kg 2.31E-01 ND ND ND ND 0 0 ND ND 0
RSF MJ ND ND ND ND ND 0 0 ND ND 0
NRSF MJ ND ND ND ND ND 0 0 ND ND 0
FW m3 5.32E-02 1.63E-05 3.19E-04 1.89E-05 1.62E-02 0 0 1.25E-04 -1E-02 0
PERE = Use of renewable primary energy excluding renewable primary energy resources used as raw materials; PERM = Use of renewable primary
energy resources used as raw materials; PERT = Total use of renewable primary energy resources; PENRE = Use of non-renewable primary energy
excluding non-renewable primary energy resources used as raw materials; PENRM = Use of non-renewable primary energy resources used as raw
materials; PENRT = Total use of non-renewable primary energy resources; SM = Use of secondary material; RSF = Use of renewable secondary fuels;
NRSF = Use of non-renewable secondary fuels; FW = Use of net fresh water
RESULTS OF THE LCA – WASTE CATEGORIES AND OUTPUT FLOWS according to EN 15804+A2:
1 m2 PENDENZATO GT
Parameter Unit A1-A3 A4 C1 C2 C3/1 C3/2 C4/1 C4/2 D/1 D/2
HWD kg 7.66E-08 1.08E-12 1.04E-10 1.25E-12 2E-10 0 0 1.78E-10 -6.91E-09 0
NHWD kg 2.53E-01 3.32E-05 3.09E-04 3.86E-05 4.97E-02 0 0 2.97E+00 -1.47E-02 0
RWD kg 2.56E-03 3.78E-07 2.42E-04 4.4E-07 7.31E-05 0 0 1.69E-05 -7.5E-03 0
CRU kg ND ND ND ND ND 0 0 ND ND 0
4 Environmental Product Declaration - Stiferite - Stiferite PENDENZATO GT
MFR kg ND ND ND ND ND 0 0 ND ND 0
MER kg ND ND ND ND ND 0 0 ND ND 0
EEE MJ ND ND ND ND 1.88E+01 0 0 4.07E-02 ND 0
EET MJ ND ND ND ND 1.72E+01 0 0 ND ND 0
HWD = Hazardous waste disposed; NHWD = Non-hazardous waste disposed; RWD = Radioactive waste disposed; CRU = Components for re-use;
MFR = Materials for recycling; MER = Materials for energy recovery; EEE = Exported electrical energy; EET = Exported thermal energy
RESULTS OF THE LCA – additional impact categories according to EN 15804+A2-optional:
1 m2 PENDENZATO GT
Parameter Unit A1-A3 A4 C1 C2 C3/1 C3/2 C4/1 C4/2 D/1 D/2
Disease
PM 1.23E-07 3.18E-10 9.01E-10 3.44E-10 9.24E-09 0 0 4.77E-09 -3.38E-08 0
incidence
IR kBq U235 eq 3.47E-01 5.71E-05 3.54E-02 6.65E-05 1.17E-02 0 0 2.34E-03 -1.1E+00 0
ETP-fw CTUe 1.04E+02 1.44E-01 4.46E-01 1.67E-01 5.76E-01 0 0 8.04E+00 -1.4E+01 0
HTP-c CTUh 4.76E-09 2.97E-12 8.21E-12 3.45E-12 4.67E-11 0 0 7.8E-11 -4.09E-10 0
HTP-nc CTUh 3.52E-07 1.85E-10 4.18E-10 2.11E-10 1.66E-09 0 0 7.6E-09 -1.93E-08 0
SQP SQP 3.8E+01 8.59E-02 1.34E-01 1E-01 3.54E-01 0 0 1.54E-01 -4.18E+00 0
PM = Potential incidence of disease due to PM emissions; IR = Potential Human exposure efficiency relative to U235; ETP-fw = Potential comparative
Toxic Unit for ecosystems; HTP-c = Potential comparative Toxic Unit for humans (cancerogenic); HTP-nc = Potential comparative Toxic Unit for humans
(not cancerogenic); SQP = Potential soil quality index
Disclaimer 1 – for the indicator “Potential Human exposure efficiency relative to U235”. This impact category deals mainly with the
eventual impact of low-dose ionizing radiation on human health of the nuclear fuel cycle. It does not consider effects due to possible
nuclear accidents, occupational exposure or radioactive waste disposal in underground facilities. Potential ionizing radiation from the
soil, radon and from some construction materials is also not measured by this indicator.
Disclaimer 2 – for the indicators “abiotic depletion potential for non-fossil resources”, “abiotic depletion potential for fossil resources”,
“water (user) deprivation potential, deprivation-weighted water consumption”, “potential comparative toxic unit for ecosystems”,
“potential comparative toxic unit for humans – cancerogenic”, “Potential comparative toxic unit for humans - not cancerogenic”,
“potential soil quality index”. The results of this environmental impact indicator shall be used with care as the uncertainties on these
results are high as there is limited experience with the indicator.
References
Standards EN 13165:2012+A2:2016 Thermal insulation products for
buildings - Factory made rigid polyurethane foam (PU)
CPR products -Specification
Regulation (EU) No.305/2011 laying down harmonised
conditions for the marketing of construction products and EN 13163
repealing Council Directive 89/106/EEC EN 13163:2012+A2:2016 Thermal insulation products for
building- factory made expanded polystyrene (EPS) products -
EN 826 Specification
EN 826:2013 Determination of Compression Behavior of
Thermal Insulation Products EN 15804
EN 15804:2012+A2:2019+AC:2021 Sustainability of
EN 1607 construction works — Environmental Product Declarations —
EN 1607: 2013 Thermal insulating products for building Core rules for the product category of construction products.
applications. Determination of tensile strength perpendicular to
faces ISO 9001
ISO 9001:2015 Quality management
EN 1609
EN 1609: Thermal insulating products for building applications. ISO 14001
Determination of short term water absorption by partial ISO 14001: 2015 Environmental management systems
immersion.
ISO 14025
EN 11925 EN ISO 14025:2011 Environmental labels and declarations —
EN 11925:2010 Reaction to fire tests. Ignitability of products Type III environmental declarations - Principles and procedures.
subjected to direct impingement of flame. Single-flame source
test. ISO 45001
ISO 45001: 2018 Occupational health and safety management
EN 12086 systems
EN 12086: 2013 Thermal insulating products for building
applications. Determination of water vapour transmission GaBi 2022
properties. GaBi 10 and DB 2022.1: Documentation of GaBi 10: Software-
System and Database for Life Cycle Engineering. Copyright,
EN 12087 TM. Stuttgart, Leinfelden-Echterdingen, 1992-2022
EN 12087:2013 Thermal insulating products for building http://www.gabi-software.com
applications. Determination of long term water absorption by
immersion. IBU 2021
Institut Bauen und Umwelt e.V.: General Instructions for the
EN 13165 EPD programme of Institut Bauen und Umwelt e.V., Version
5 Environmental Product Declaration - Stiferite - Stiferite PENDENZATO GT
2.0, Berlin: Institut Bauen und Umwelt e.V., 2021 n.183 del
www.ibu-epd.com 06-08-2022
https://www.mite.gov.it/notizie/novita-sui-criteri-minini-
IBU PCR Part A ambientali-cam
Product Category Rules for Building-Related Products and
Services. Part A: Calculation Rules for the Life Cycle REACH
Assessment and Requirements on the Project Report according REACH Registration, Evaluation, Authorization and Restriction
to EN 15804+A2:2019; V1.2, 11/2021 of Chemical, 2007
IBU PCR Part B Ordinance on Biocide Products
PCR Guidance-Texts for Building-Related Products and Regulation (eu) n. 528/2012 of the European Parliament and of
Services; Part B: Requirements on the EPD for Insulating the Council of 22 May 2012 concerning the making available on
materials made of foam plastics; Institute Construction and the market and use of biocidal products Text with EEA
Environment e.V. (IBU). Version 01.2019 relevance
https://epd-online.com
REMADE IN ITALY
PANGPP 2022 Certificate No.1245/001 for Stiferite Rev. n. 0 18 November
Piano d' Azione Nazionale sul Green Public Procurement 2021
(PANGPP) – Decreto Ministeriale n. 256 del 23-06-2022
Gazzetta Ufficiale della Repubblica Italiana, Serie Generale STIFERITE LCA tool background report v 2.3 (03-06-2022)
6 Environmental Product Declaration - Stiferite - Stiferite PENDENZATO GT
Publisher
Institut Bauen und Umwelt e.V. +49 (0)30 3087748- 0
Hegelplatz 1 info@ibu-epd.com
10117 Berlin www.ibu-epd.com
Germany
Programme holder
Institut Bauen und Umwelt e.V. +49 (0)30 3087748- 0
Hegelplatz 1 info@ibu-epd.com
10117 Berlin www.ibu-epd.com
Germany
Author of the Life Cycle Assessment
Sphera Solutions GmbH +49 711 341817-0
Hauptstraße 111- 113 info@sphera.com
70771 Leinfelden-Echterdingen www.sphera.com
Germany
Owner of the Declaration
Stiferite +39 049 8997911
Viale Navigazione Interna 54 info@stiferite.com
35129 Padova www.stiferite.com
Italy
7 Environmental Product Declaration - Stiferite - Stiferite PENDENZATO GT
