ENVIRONMENTAL PRODUCT DECLARATION
as per ISO 14025 and EN 15804+A1
Owner of the Declaration Troldtekt A/S
Programme holder Institut Bauen und Umwelt e.V. (IBU)
Publisher Institut Bauen und Umwelt e.V. (IBU)
Declaration number EPD-TRO-20220048-ICA2-EN
Issue date 11.04.2022
Valid to 06.04.2027
Acoustic panels - unpainted
Troldtekt 25 mm Natural Grey
based on FUTURECEM
www.ibu-epd.com | https://epd-online.com
Umwelt Produktdeklaration Name des Herstellers – Name des Produkts
1. General Information
Troldtekt A/S Troldtekt 25 mm Natural Grey
based on FUTURECEM - unpainted
Programme holder Owner of the declaration
IBU – Institut Bauen und Umwelt e.V. Troldtekt A/S
Hegelplatz 1 Sletvej 2 A
10117 Berlin 8310 Tranbjerg
Germany Denmark
Declaration number Declared product / declared unit
EPD-TRO-20220048-ICA2-EN Acoustic panel "Natural Grey FUTURECEM" - 1 m2, 25
mm thickness - unpainted
This declaration is based on the product Scope:
category rules: This declaration represents the production, supply,
Wood cement - Mineral-bonded wooden composites, mounting, use, dismantling and disposal of 1 m2 (25
01.2019 mm thickness) of grey composite cement-bonded
(PCR checked and approved by the SVR) wood wool acoustic panel "Natural Grey
FUTURECEM", produced by Troldtekt A/S, with a
reference service life of 50 years. The production
Issue date
facility is located in Jutland, Denmark. Three scenarios
11.04.2022
represent its use in indoor conditions in Denmark,
Sweden and Germany.
Valid to
06.04.2027
The owner of the declaration shall be liable for the
underlying information and evidence; the IBU shall not
be liable with respect to manufacturer information, life
cycle assessment data and evidences.
The EPD was created according to the specifications
of EN 15804+A1. In the following, the standard will be
simplified as EN 15804.
Verification
The standard EN 15804 serves as the core PCR
Independent verification of the declaration and data
according to ISO 14025:2011
Dipl. Ing. Hans Peters internally x externally
(chairman of Institut Bauen und Umwelt e.V.)
Dr. Alexander Röder Ms Jane Anderson
(Managing Director Institut Bauen und Umwelt e.V.)) (Independent verifier)
2. Product
2.1 Product description/Product definition For the application and use, the respective national
Troldtekt Natural Grey FUTURECEM acoustic panels provisions apply.
are some of the leading and preferred solutions for
creating a good indoor sound environment. They are 2.2 Application
sold in various thicknesses (20-35 mm) and The panels are installed on the ceilings and walls in
dimensions (width: 600 mm, lengths: 600/1200/2400 offices, businesses, schools, institutions, cultural sites,
mm or width: 625 mm, lengths: 625/1250/2500 sports centres, swimming pools and private homes.
mm ). The panels can be unpainted or painted in a
wide variety of colours. 2.3 Technical Data
The table below indicates the technical specifications
For the placing on the market of the product in the of the panels in accordance with EN 13168, the
European Union/European Free Trade Association standard for cement-bonded wood wool and double-
(EU/EFTA) (with the exception of Switzerland) layer panels with cement-bonded wood wool, and EN
Regulation (EU) No. 305/2011 applies. The product 13964, the standard for suspended ceilings.
needs a declaration of performance taking into
consideration EN 13964:2014, Suspended ceilings.
Requirements and test methods, and the CE-marking.
2 Environmental Product Declaration Troldtekt A/S – Troldtekt 25mm Natural Grey FUTURECEM - unpainted
The wood wool is mixed together with Portland
composite cement, water, and additives. The mixture is
cast and cured using a heat press and dried with a
biomass-fired oven. The cast panel is milled to remove
any material in excess and cut edges. After
Technical specifications of the product covered in approximately 4 weeks of curing, the panel can be
this EPD painted before being stored on a pallet and packaged
Name Value Unit to be transported to central distribution warehouses.
Gross density 463 kg/m3
Grammage 11.59 kg/m2 2.7 Environment and health during
Thermal conductivity acc. to EN manufacturing
0.076 W/(mK)
13168:2012+A1:2015 Troldtekt is following its working environment closely.
Water vapour diffusion resistance Both the physical working environment and sickness
- -
factor acc. to DIN 4108-4 absence are closely monitored. It is an ongoing
Sound absorption coefficient (only with process involving both leaders and factory workers.
reference to the corresponding - %
component design) 2.8 Product processing/Installation
Light reflection (measured by DELTA 26.3 - Installation instructions are available here:
Light and Optics 70.8 % https://www.troldtekt.com/Installation
Reaction to fire B/S1/d0
2.9 Packaging
The product is packaged with polyethylene plastic film
and cardboard. The packaging material can be easily
Performance data of the product in accordance with
sorted and treated in dedicated waste recycling
the declaration of performance with respect to its
channels. The packaged product is delivered on a
essential characteristics according to EN
returnable wood pallet.
13168:2012+A1:2015, Thermal insulation products for
buildings. Factory made wood wool (WW) products.
Specification, and EN 13964:2014, Suspended
2.10 Condition of use
ceilings. Requirements and test methods.
Conditions of use are detailed
here: https://www.troldtekt.com/Installation/Use_and_
2.4 Delivery status
maintenance
The panel is usually distributed in length of 600, 1200
or 2400 mm by 600 mm width or in length of 625, 1250
2.11 Environment and health during use
or 2500 mm by 625 mm width. It comes in three
Environmental and ecotoxicity risks from exposure to
thicknesses: 20, 25 and 35 mm. Additionally, several
Troldtekt panel products during use have been
density ranges are available: Coarse, Fine, Ultra-Fine
assessed and found eligible to the following
and Extreme-Fine causing different densities (388-428
certification schemes:
kg/m3). The panels are normally delivered in packs of
80 units on pallets.  Finnish M1 classification
 Danish Indoor Climate
2.5 Base materials/Ancillary materials  Cradle to Cradle
The composition of the finished product is a mix of
wood wool (31.9 %), Portland composite cement (62.2
These certificates can be accessed
%), water (4.5 %), as well as water glass (<1 %) and
here: https://www.troldtekt.com/Web-
accelerator (<1 %). The composition is at dry basis at
tools/Downloads/Certificates-and-tests
the factory gate, as most of the water has evaporated
during drying, but water remains bound to the wood
2.12 Reference service life
fibre and cement paste (hydrated cement).
The technical service life of the panel is superior to 50
years. This EPD refers to the service lifetime indicated
This product/article/at least one partial article contains
by the BBSR table for the material 353.311 of type
substances listed in the candidate list (date:
“Holzbekleidungen: Holz, Holzwerkstoff und
17.01.2022) exceeding 0.1 percentage by mass: No
Mehrschichtleichtbauplatten”.
This product/article/at least one partial article contains
Because the panel is used in a building, in this EPD its
other CMR substances in categories 1A or 1B which
reference service life is limited by the expected service
are not on the candidate list, exceeding 0.1 percentage
life of the building, which is commonly accepted as 50
by mass: No
years, at least as LCA timeframe.
Biocide products were added to this construction
There is no influence of the ageing of the material on
product or it has been treated with biocide products
its technical performance.
(this then concerns a treated product as defined by the
(EU) Ordinance on Biocide Products No. 528/2012):
2.13 Extraordinary effects
No
Fire
2.6 Manufacture
Information on the fire performance according to EN
Norway spruce logs from local forests (with a moisture
13168.
content of about 65-70 %) are received and the bark is
removed. The wood is stored for approximately six
Fire protection
months until the moisture content in the wood drops to
Name Value
29 %. The wood is then shredded to produce wool.
Building material class B
3 Environmental Product Declaration Troldtekt A/S – Troldtekt 25mm Natural Grey FUTURECEM - unpainted
Burning droplets d0
Smoke gas development S1 2.15 Disposal
The product may be composted, thermally treated with
Water energy recovery, or landfilled.
No information on the product performance under the
unforeseeable influence of water is available. European Waste Code: 10 13 11 (wastes from
cement-based composite materials)
Mechanical destruction
No information on the product performance under Painted panels must be incinerated at end-of-life.
unforeseeable mechanical destruction is available.
Additional information on disposal
2.14 Re-use phase options: https://www.troldtekt.com/environment-and-
Currently, Troldtekt panels undergo thermal treatment csr/product-life-cycle/recycling/
with energy recovery. Composting is also possible.
2.16 Further information
Additional information on recycling For additional information on technical specifications,
options: https://www.troldtekt.com/~/media/Files/Info% you may consult the Declaration Of
20sheets/English/Troldtekt_Recycling%20instructions Performance: https://www.troldtekt.com/Web-
%20pdf.pdf tools/Downloads/DoPs
3. LCA: Calculation rules
3.1 Declared Unit
The functional unit is 1 m2 of acoustic panel, in 25 mm 3.6 Data quality
thickness, corresponding to 11.59 kg of material with Statistical representativeness
unpainted finish, mounted on the ceiling, with a The statistical representativeness of the product
reference service life of 50 years. system is very good. The input and output data
samples used to build inventories are based on the
Declared unit entirety of the annual production of panels in 2020 and
Name Value Unit is verified by a third party. Such representativeness is
Declared unit 1 m2 also valid for the production of Portland composite
Gross density 463 kg/m3 cement (FUTURECEM), whose EPD was published in
Grammage 11.59 kg/m2 2019 and audited in 2021. The EPD for the paint used
Layer thickness 0.025 m was published in 2018.
Temporal, geographical and technological
representativeness
3.2 System boundary All data strictly related to the cement production is
Cradle to grave technologically, temporally, and geographically
representative. The cement production data is less
3.3 Estimates and assumptions than 5 years old. The data used to model the
Assumptions are described occasionally throughout foreground inventory of acoustic panels dates from the
the section "LCA: Calculation rules". production year of 2020. As for secondary data, some
of the ecoinvent datasets are less than 3 years old.
3.4 Cut-off criteria
The cut-off criterion is applied according to EN 3.7 Period under review
15804 Section 6.3.5 and PCR part A Section 5.6. The primary data concerned with the manufacture (A1-
All inputs and outputs for which data are available are A3) relates to the production year 2020 and the data
included in the LCA model. Data gaps are filled with are based on the volumes produced on an annual
conservative assumptions from average data (when basis.
available) or with generic data and are documented
accordingly. 3.8 Allocation
The following product flows have been omitted Allocation of production data to the multiple produced
according to the 1% cut-off rule: types of panels (with the same functional unit) is
 Wooden pallet to transport the product performed based on the rules provided in EN 15804.
Sub-processes associated to painting have especially
 Capital infrastructure (factory)
been allocated to the painted panels. Data such as
 Allocation of burden from wood logging to
waste generation and packaging have been allocated
residual wood fractions to the entire production volume of panels in Troldtekt.
The only case of co-produced outputs is associated to
wood logging. However, the environmental load is
evenly distributed over all its co-products, such as
3.5 Background data
logs, energy wood, and bark.
Two types of data source are used as secondary data:
 Product-specific EPDs for the manufacture
3.9 Comparability
and supply of Portland composite cement and
Basically, a comparison or an evaluation of EPD data
water-based paint
is only possible if all the data sets to be compared
 Database ecoinvent v.3.6 cut-off were created according to EN 15804 and the building
context, respectively the product-specific
characteristics of performance, are taken into account.
4 Environmental Product Declaration Troldtekt A/S – Troldtekt 25mm Natural Grey FUTURECEM - unpainted
The used background database is ecoinvent v.3.6 cut-
off
4. LCA: Scenarios and additional technical information
Manufacture (A1-A3) Capacity utilisation volume factor 1 -
Data
Primary data is third-party verified and based on the
production year 2020, within the facilities of Troldtekt
A/S in Jutland (Denmark). Installation into the building (A5)
Name Value Unit
End-of-waste state and use of by-products Electricity consumption 0.060 kWh
For all processes supplying a residual material/waste Material loss (plastic film) 0.007 kg
that originates the end-of-life phase of a product to the Material loss (cardboard) 0.032 kg
product system to be used as input, the polluter-pay
principle “100:0” is used. Some wooden by-products Use phase (B1)
generated during manufacture in Troldtekt end up as Before distribution and during the use phase (B1), the
soil improvers externally (reaching end-of-waste state), carbonation of the cement contained in the panel,
and thus their biogenic carbon leaves Troldtekt's during use, is accounted for. Based on laboratory
system boundary. measurement, the panel will absorb up to 140 grams of
carbon dioxide per kilogram of cement. Normalized to
Wind-certified electricity the reference flow, this corresponds to an uptake of
All the electricity used to produce the panels in Module approximately 0.7 kilograms of carbon dioxide by the
A3 originates from Danish wind power, for which a end of the service lifetime, including the uptake in A3.
certificate ensures the origin. It originates from a 1-3
MW offshore wind turbine, with transformation, Maintenance (B2)
transmission and distribution losses and is modelled As the panel does not require any maintenance except
correspondingly. for the occasional dusting, no maintenance module
(B2) is considered.
Carbon balance
Biogenic: Absorption of biogenic CO by the purchased
2 Name Value Unit
wood has been considered in A1. Some of it is
released again during production in A3, some ends up
Repair, replacement, refurbishment (B3, B4, B5)
sequestered in soil, while the majority of the remaining
As the technical service life of the panel is superior to
biogenic CO , 7.15 kg, is retained in the finished
2 the assumed service life of the building (50 years), no
product and emitted during end-of-life incineration in
repair (B3), replacement (B4) or refurbishment (B5)
C4.
steps are considered.
Fossil: Absorption of some fossil CO , originating from
2
the calcination of limestone during cement production,
happens when the cement is mixed with water in A3. A Name Value Unit
majority is absorbed during the use phase B1, and all
the absorbed fossil CO is finally emitted during end- Replacement (B4) / Refurbishment (B5)
2
of-life incineration in C4. Name Value Unit
Distribution to site (A4) and mounting (A5) Information about reference service life is detailed in
To consider the main geographical variants of the life 2.12.
cycle of Troldtekt Natural Grey FUTURECEM panels,
three scenarios are developed, where the product is Reference service life
supplied, mounted, used and discarded in Aarhus Name Value Unit
(Denmark), Hamburg (Germany) and Malmö Reference service life (according to 50 a
(Sweden). An additional 50 km from the local ISO 15686-1, -2, -7 and -8)
warehouse to construction site is assumed. Life Span (according to BBSR) 50 a
Life Span according to the
75 a
manufacturer
Transport to the building site (A4)
Name Value Unit Operational energy use (B6) and Operational water
Litres of fuel 26.8 l/100km use (B7)
Transport distance to Denmark 160 km Name Value Unit
Transport distance to Germany 370 km Water consumption - m3
Transport distance to Sweden 394 km Electricity consumption - kWh
Transport distance from warehouse to Other energy carriers - MJ
local construction sites in 50 km Equipment output - kW
Denmark/Germany/Sweden
Capacity utilisation (including empty End of life (C1-C4)
85 %
runs) Name Value Unit
Gross density of products transported 463 kg/m3 Electricity use (for un-mounting) 0.060 kWh
5 Environmental Product Declaration Troldtekt A/S – Troldtekt 25mm Natural Grey FUTURECEM - unpainted
Transport (to material sorting facility) 50 km
Collected as mixed construction waste 11.59 kg
Energy recovery 3.64 kg
Energy recovery efficiency 10 %
Energy recovered 7.42 MJ
The panel is un-mounted at the end of its reference
service life and driven to the regional waste
incineration plant. Energy is recovered from the wood
part of the panel at 10 % efficiency.
Reuse, recovery and/or recycling potentials (D),
relevant scenario information
Name Value Unit
Electricity 1.76 MJ
Heat 5.66 MJ
The energy substituted from incineration of the panel's
wood component in C4 is considered to be a split of
the Danish electricity grid mix (for electricity) and
natural gas (for heat).
Details on possible disposal routes
Aalborg Portland cement factory utilizes dust and
offcuts from the Troldtekt factory as a raw material in
new cement, i.e. in the technical circle. During
incineration in the cement kiln, the wood content in the
cement-bonded wood wool panels replaces fossil
fuels, while the cement ends up as a raw material in
new cement, replacing virgin raw materials and heavy
fossil fuels, thereby avoiding a significant amount of
CO emissions. This scheme of wood wool waste as a
2
raw material can be scaled for construction site and
demolition waste. It will be gradually rolled out to all of
Denmark in the period 2021-2023. Once Denmark has
documented economic and environmental benefits to
be gained by including wood wool waste in the
production of new cement rather than going to waste
incineration or landfill, dialogue with municipalities and
local cement producers in the primary markets of
Troldtekt is initiated to facilitate similar schemes
regionally or nationally.
6 Environmental Product Declaration Troldtekt A/S – Troldtekt 25mm Natural Grey FUTURECEM - unpainted
5. LCA: Results
Note: Global Warming Potential (GWP) indicator includes CO of both biogenic and fossil origin.
2
Also, GWP results for Troldtekt Natural Grey FUTURECEM (unpainted) for other delivery scenarios in
respectively Germany and Sweden, are 2.27E-1 kg CO and 2.40E-1 kg CO .
2 2
DESCRIPTION OF THE SYSTEM BOUNDARY (X = INCLUDED IN LCA; MND = MODULE NOT DECLARED;
MNR = MODULE NOT RELEVANT)
BENEFITS AND
CONSTRUCTI LOADS
PRODUCT STAGE ON PROCESS USE STAGE END OF LIFE STAGE BEYOND THE
STAGE SYSTEM
BOUNDARIES
7 Environmental Product Declaration Troldtekt A/S – Troldtekt 25mm Natural Grey FUTURECEM - unpainted
lairetam
waR
ylppus tropsnarT
gnirutcafunaM
eht
morf
tropsnarT
etis
eht
ot
etag
ylbmessA esU
ecnanetniaM
riapeR
tnemecalpeR tnemhsibrufeR
ygrene
lanoitarepO esu
retaw
lanoitarepO esu
noitcurtsnoc-eD
noitilomed tropsnarT
gnissecorp
etsaW
lasopsiD -esueR -yrevoceR -gnilcyceR laitnetop
A1 A2 A3 A4 A5 B1 B2 B3 B4 B5 B6 B7 C1 C2 C3 C4 D
X X X X X X MND MNR MNR MNR MND MND X X MND X X
RESULTS OF THE LCA - ENVIRONMENTAL IMPACT according to EN 15804+A1: 1 m2 Natural Grey
FUTURECEM, 25 mm, unpainted, delivered and used in Denmark
Parameter Unit A1-A3 A4 A5 B1 C1 C2 C4 D
GWP [kg CO2-Eq.] -1.37E+0 1.14E-1 2.41E-1 -5.34E-1 6.50E-4 9.59E-2 7.87E+0 -9.69E-1
ODP [kg CFC11-Eq.] 1.99E-7 2.08E-8 1.14E-8 0.00E+0 2.81E-10 1.75E-8 6.52E-9 -5.36E-8
AP [kg SO2-Eq.] 1.23E-2 2.30E-4 7.24E-4 0.00E+0 1.59E-6 1.94E-4 5.38E-4 -2.01E-3
EP [kg (PO4)3--Eq.] 5.46E-3 4.73E-5 3.93E-4 0.00E+0 8.86E-7 3.98E-5 2.34E-4 -1.49E-3
POCP [kg ethene-Eq.] 7.19E-4 1.52E-5 4.25E-5 0.00E+0 8.88E-8 1.28E-5 4.22E-5 -1.16E-4
ADPE [kg Sb-Eq.] 5.24E-5 3.11E-6 4.92E-6 0.00E+0 1.82E-8 2.61E-6 7.10E-7 -2.60E-6
ADPF [MJ] 3.59E+1 1.73E+0 2.23E+0 0.00E+0 4.20E-2 1.46E+0 6.50E-1 -1.36E+1
GWP = Global warming potential; ODP = Depletion potential of the stratospheric ozone layer; AP = Acidification potential of land and water; EP =
Caption Eutrophication potential; POCP = Formation potential of tropospheric ozone photochemical oxidants; ADPE = Abiotic depletion potential for non-
fossil resources; ADPF = Abiotic depletion potential for fossil resources
RESULTS OF THE LCA - INDICATORS TO DESCRIBE RESOURCE USE according to EN 15804+A1: 1 m2
Natural Grey FUTURECEM, 25 mm, unpainted, delivered and used in Denmark
Parameter Unit A1-A3 A4 A5 B1 C1 C2 C4 D
PERE [MJ] 6.83E+1 2.44E-2 4.50E-1 0.00E+0 3.91E-2 2.06E-2 8.59E+0 -6.34E+0
PERM [MJ] 7.47E+1 0.00E+0 0.00E+0 0.00E+0 0.00E+0 0.00E+0 0.00E+0 0.00E+0
PERT [MJ] 1.43E+2 2.44E-2 4.50E-1 0.00E+0 3.91E-2 2.06E-2 8.59E+0 -6.34E+0
PENRE [MJ] 3.63E+1 1.73E+0 2.23E+0 0.00E+0 4.20E-2 1.46E+0 6.50E-1 -1.36E+1
PENRM [MJ] 0.00E+0 0.00E+0 0.00E+0 0.00E+0 0.00E+0 0.00E+0 0.00E+0 0.00E+0
PENRT [MJ] 3.63E+1 1.73E+0 2.23E+0 0.00E+0 4.20E-2 1.46E+0 6.50E-1 -1.36E+1
SM [kg] 1.35E+0 0.00E+0 2.73E-3 0.00E+0 0.00E+0 0.00E+0 0.00E+0 0.00E+0
RSF [MJ] 7.89E+0 0.00E+0 0.00E+0 0.00E+0 0.00E+0 0.00E+0 0.00E+0 0.00E+0
NRSF [MJ] 8.34E+0 0.00E+0 0.00E+0 0.00E+0 0.00E+0 0.00E+0 0.00E+0 0.00E+0
FW [m³] 1.72E-2 2.96E-4 2.20E-3 0.00E+0 1.19E-5 2.49E-4 2.86E-4 -1.86E-3
PERE = Use of renewable primary energy excluding renewable primary energy resources used as raw materials; PERM = Use of
renewable primary energy resources used as raw materials; PERT = Total use of renewable primary energy resources; PENRE = Use of
non-renewable primary energy excluding non-renewable primary energy resources used as raw materials; PENRM = Use of non-
Caption
renewable primary energy resources used as raw materials; PENRT = Total use of non-renewable primary energy resources; SM = Use
of secondary material; RSF = Use of renewable secondary fuels; NRSF = Use of non-renewable secondary fuels; FW = Use of net fresh
water
RESULTS OF THE LCA – WASTE CATEGORIES AND OUTPUT FLOWS according to EN 15804+A1:
1 m2 Natural Grey FUTURECEM, 25 mm, unpainted, delivered and used in Denmark
Parameter Unit A1-A3 A4 A5 B1 C1 C2 C4 D
HWD [kg] 4.74E-2 1.76E-3 7.11E-2 0.00E+0 5.40E-5 1.48E-3 1.50E-3 -5.92E-2
NHWD [kg] 1.63E+0 1.21E-1 4.24E-1 0.00E+0 1.12E-3 1.02E-1 6.31E-2 -2.02E+0
RWD [kg] 7.82E-5 1.19E-5 8.28E-6 0.00E+0 5.78E-7 9.99E-6 5.06E-6 -2.45E-5
CRU [kg] 0.00E+0 0.00E+0 0.00E+0 0.00E+0 0.00E+0 0.00E+0 0.00E+0 0.00E+0
MFR [kg] 4.86E-3 0.00E+0 0.00E+0 0.00E+0 0.00E+0 0.00E+0 0.00E+0 0.00E+0
MER [kg] 1.05E-2 0.00E+0 0.00E+0 0.00E+0 0.00E+0 0.00E+0 0.00E+0 0.00E+0
EEE [MJ] 0.00E+0 0.00E+0 0.00E+0 0.00E+0 0.00E+0 0.00E+0 1.76E+0 0.00E+0
EET [MJ] 0.00E+0 0.00E+0 0.00E+0 0.00E+0 0.00E+0 0.00E+0 5.66E+0 0.00E+0
HWD = Hazardous waste disposed; NHWD = Non-hazardous waste disposed; RWD = Radioactive waste disposed; CRU = Components
Caption for re-use; MFR = Materials for recycling; MER = Materials for energy recovery; EEE = Exported electrical energy; EEE = Exported
thermal energy
6. LCA: Interpretation
The estimated impact results are only relative foreground processes. Global Warming Potential net
statements that do not indicate the end points of the emissions share is much larger in C4 than in A1-A3
impact categories, exceeding threshold values, safety (see why in chart (2)), while other impact categories in
margins or risks. module D, in general, are avoided in the waste system
owing to the incineration of end-of-life panels and
Two charts are presented: (1) with the standard substitution of natural gas and Danish electricity mix.
lifecycle impact categories displaying the share of C4 also slightly follows emissions of compounds
impacts across all lifecycle stages, and (2) displaying associated to other impact categories. A relatively
the total carbon balance of the Troldekt product's inefficient transportation of end-of-life panels to waste
lifecycle system. incineration causes emissions in especially Abiotic
depletion of non-fossil resources, Depletion of
Impacts from the A1-A3 modules are dominant in the stratospheric ozone, and Photochemical ozone
life cycle of the Troldtekt Natural Grey FUTURECEM formation.
panel products. This is primarily caused by the
acquisition and use of cement and wood in the
The embodied emissions associated to the raw is re-emitted in C4. CO emissions ocuring in the
2-eq
materials (primarily cement) are the main cause of remaining modules are negligible.
impacts, especially in terms of net Global Warming
Potential, with 4.85 kg CO for cement followed by The amount of wood stored in the product refers to a
2-eq
minor impacts from additives. In general, direct negative contribution to Global Warming Potential,
emissions from the Troldtekt production site are reducing the share of Global Warming Potential in A1-
relatively small. Abiotic depletion of fossil resources A3. This is due to the sequestration of biogenic carbon
appears from the burden of producing cement using of wood during tree growth. The sequestered carbon
fossil raw material such as limestone and to a large does not contribute to global warming as long as it is
extent fossil fuels. In terms of carbon balance, biogenic stored in the biomass.
CO in A1-A3 offsets nearly all the fossil CO
2 2
emissions in A1-A3. All biogenic CO sequestered in
2
A1-A3 and some fossil CO taken up in A1-A3 and B1
2
8 Environmental Product Declaration Troldtekt A/S – Troldtekt 25mm Natural Grey FUTURECEM - unpainted
The clinker (cement) production is the most critical
Summary process of the Troldtekt product system, but
Within the cradle to grave, the following aspects have inaccuracies around the amount used will not
been identified as major contributors, mainly in the invalidate the present conclusions.
categories Global Warming Potential and Abiotic
depletion of fossil resources: Notably, by introducing more up-to-date LCA datasets
for the grey cement applied, or introducing cements
 Emissions from the clinker production from with less carbon footprint into production could lead to
material significant reductions of especially the Global Warming
Potential indicator.
 Emissions from the clinker production from
fuel
 Substituted emissions from end of life
incineration
7. Requisite evidence
Technological Institute under DANAK accreditation
7.1 Testing of substances used 392. Report no. MAIC-2019-1418. Reporting of
A detailed assessment of substances used was measured concentrations in toluene equivalents
conducted by a DAkkS-accredited laboratory, based according to EN 16516. This test is the basis for the
on a sample (prepared according to EN 15443), Finish M1 Material certificate as well as the Danish
available in the Test Report 2018P216294, using Indoor Climate labelling certificate.
inductively coupled plasma mass spectrometry (EN
16171) and X-ray fluorescence (EN 15309), for the AgBB overview of results (28 days [µg/m³])
following: Name Value Unit
 Heavy metals (cadmium, mercury, etc.) TVOC (C6 - C16) 12 μg/m3
 and other elements Sum SVOC (C16 - C22) 0 - 5 μg/m3
VOC without NIK 0 - 5 μg/m3
Carcinogenic Substances 1 μg/m3
7.2 Leaching
No leaching measurement was conducted according
AgBB overview of results (3 days [µg/m³])
to EN 717-1.
Name Value Unit
TVOC (C6 - C16) - μg/m3
Sum SVOC (C16 - C22) - μg/m3
7.3 VOC emissions
R (dimensionless) - -
Testing for VOC emissions has been conducted in
VOC without NIK - μg/m3
accordance with EN ISO 16000-6. Analysis of the air
Carcinogenic Substances - μg/m3
sampled on Tenax was performed at the Danish
8. References
Standards DIN 52612-2, Testing of thermal insulating materials;
determination of thermal conductivity by means of the
guarded hot plate apparatus; conversion of the
AgBB measured values for building applications. 1 June 1984
AgBB, Ausschuss zur gesundheitlichen Bewertung von
Bauprodukten (Committee for Health-related DIN EN ISO 14025
Evaluation of Building Products) DIN EN ISO 14025:2011, Environmental labels and
declarations – Type III environmental
BBSR declarations – Principles and procedures, German and
BBSR, Bundesinstitut für Bau-, Stadt- und English versions EN ISO 14025:2011
Raumforschung (Federal Institute for Research on
Building, Urban Affairs and Spatial Development). EN 13168
BBSR table: EN 13168:2012+A1:2015, Thermal insulation products
https://www.nachhaltigesbauen.de/fileadmin/pdf/baust for buildings. Factory made wood wool (WW) products.
off_gebauededaten/BNB_Nutzungsdauern_von_Bautei Specification
len_2017-02-24.pdf
EN 13964
DIN 4108-4 EN 13964:2014, Suspended ceilings. Requirements
DIN 4108-4:2017-03, Thermal insulation and energy and test methods
economy in buildings - Part 4: Hygrothermal design
values EN 15309
EN 15309:2007, Characterization of waste and soil.
DIN 52612-2 Determination of elemental composition by X-ray
fluorescence
9 Environmental Product Declaration Troldtekt A/S – Troldtekt 25mm Natural Grey FUTURECEM - unpainted
ISO 16000-6:2011, Indoor air - Part 6: Determination of
EN 15443 volatile organic compounds in indoor and test chamber
EN 15443:2011, Solid recovered fuels. Methods for the air by active sampling on Tenax TA sorbent, thermal
preparation of the laboratory sample desorption and gas chromatography using MS or MS-
FID
EN 15804
EN 15804:2012, EN 15804:2012+A1 2013, Product Category Rule A
Sustainability of construction works – Environmental Product Category Rule A, IBU, 2019, Part A,
Product Declarations – Core rules for the product Calculation Rules for the Life Cycle Assessment and
category of construction products. Requirements on the Project Report. v.1.8. IBU, 2019.
EN 16171 Product Category Rule B
EN 16171:2016, Sludge, treated biowaste and soil. Product Category Rule B, IBU, 2019, Part B,
Determination of elements using inductively coupled Requirements on the EPD for Wood cement - Mineral-
plasma mass spectrometry (ICP-MS) bonded wooden composites. v.1.7. IBU, 2019.
EN 16449 Regulation (EU) No. 305/2011
EN 16449:2014, EN 16449:2014, Wood and wood-
based products - Calculation of the biogenic carbon
content of wood and conversion to carbon dioxide Further References
EN 16516 General Programme Instructions, IBU 2021
EN 16516:2017+A1:2020, Construction products: General Instructions for the EPD programme of Institut
Assessment of release of dangerous substances. Bauen und Umwelt e.V. Version 2.0, Berlin: Institut
Determination of emissions into indoor air Bauen und Umwelt e.V., 2021. www.ibu-epd.com
EN 717-1 Software/database
EN 717-1:2004, Wood-based Panels – Determination OneClick LCA software, Pre-verified EPD tool,
of Formaldehyde Release – Formaldehyde emission Bionova: https://www.oneclicklca.com/
by the chamber method
Database: Ecoinvent v.3.6. cut-off (2019)
European Waste Code: 10 13 11 https://ecoinvent.org/the-ecoinvent-database/
(wastes from cement-based composite materials)
ISO 16000-6
10 Environmental Product Declaration Troldtekt A/S – Troldtekt 25mm Natural Grey FUTURECEM - unpainted
Publisher
Institut Bauen und Umwelt e.V. Tel +49 (0)30 3087748- 0
Hegelplatz 1 Fax +49 (0)30 3087748- 29
10117 Berlin Mail info@ibu-epd.com
Germany Web www.ibu-epd.com
Programme holder
Institut Bauen und Umwelt e.V. Tel +49 (0)30 - 3087748- 0
Hegelplatz 1 Fax +49 (0)30 – 3087748 - 29
10117 Berlin Mail info@ibu-epd.com
Germany Web www.ibu-epd.com
Author of the Life Cycle
Assessment Tel 98777223
Aalborg Portland Fax 80815733
Rørdalsvej 44 Mail
92200 Aalborg Ø stefan.e.danielsson@cementirhol
Denmark ding.it
Web www.aalborgportland.dk
Owner of the Declaration
Troldtekt A/S Tel +45 8747 8100
Sletvej 2A Fax +45 8747 8111
8310 Tranbjerg J Mail sales@troldtekt.dk
Denmark Web https://www.troldtekt.com
