ENVIRONMENTAL PRODUCT DECLARATION
as per ISO 14025 and EN 15804+A2
Owner of the Declaration Unilin BV, division flooring
Publisher Institut Bauen und Umwelt e.V. (IBU)
Programme holder Institut Bauen und Umwelt e.V. (IBU)
Declaration number EPD-UNI-20230478-IBC1-EN
Issue date 15.01.2024
Valid to 14.01.2029
Multi-layer parquet flooring
Unilin BV, division flooring
www.ibu-epd.com | https://epd-online.com
1. General Information
Unilin BV, division flooring Multi-layer parquet flooring
Programme holder Owner of the declaration
IBU – Institut Bauen und Umwelt e.V. Unilin BV, division flooring
Hegelplatz 1 Ooigemstraat 3
10117 Berlin 8710 Wielsbeke
Germany Belgium
Declaration number Declared product / declared unit
EPD-UNI-20230478-IBC1-EN 1m² of Multilayer parquet flooring (representing weighted average on sales
with average thickness of 13.25 mm and average mass of 9.55 kg/m²).
This declaration is based on the product category rules: Scope:
Floor coverings, 01.08.2021 This declaration is an environmental product declaration according to ISO
(PCR checked and approved by the SVR) 14025 - Type III and EN 15804+A2 describing the environmental
performances of 1m² of a 3-layer parquet flooring produced by Unilin BV,
division Flooring in the production plant in Malaysia - Syarikat Malaysia
Issue date Wood Industries Sdn. Bhd, 864 - V Syarikat.
15.01.2024
The product is available with 3 brand names:
• Quickstep
Valid to • Pergo
• Unilin
14.01.2029
In this EPD the LCA results for HDF or Hevea core products average sales
are declared (average mass of 9,55 kg/m² and average thickness of 13,25
mm).
The owner of the declaration shall be liable for the underlying information
and evidence; the IBU shall not be liable with respect to manufacturer
information, life cycle assessment data and evidences.
The EPD was created according to the specifications of EN 15804+A2. In
the following, the standard will be simplified as EN 15804.
Verification
Dipl.-Ing. Hans Peters The standard EN 15804 serves as the core PCR
(Chairman of Institut Bauen und Umwelt e.V.) Independent verification of the declaration and data according to ISO
14025:2011
internally X externally
Florian Pronold Dr. Frank Werner,
(Managing Director Institut Bauen und Umwelt e.V.) (Independent verifier)
1 Environmental Product Declaration - Unilin BV, division flooring - Multi-layer parquet flooring
2. Product
• 1820mm x 190mm x 12,5mm
2.1 Product description/Product definition
This environmental product declaration refers to the production 2.5 Base materials/Ancillary materials
of 1m² multi-layer parquet flooring (MLP). The multilayer flooring elements have the composition
presented below:
The multilayer parquet is produced in the Unilin production
• Wood layers (surface + Core layer solid or HDF +
facilities in Malaysia and meets the
backing) : 94% - 96%
requirements of EN 14342 and EN 13489. The panels have a
• Glue : 3% - 5%
mechanical and patented connection (uniclic and multifit).
• Finishing : 1%
The surface layer of the product consists of layers UV-curing
Core layer
acrylic layer or layers of UV-curing oil.
The core of the multilayer flooring elements consists of wooden
The multi-layer parquet contains at least 70% PEFC certified
core boards of a High-density fiberboard or wood.
wood.
For the placing on the market of the product in the European
Surface layer
Union/European Free Trade Association (EU/EFTA) (with the
On top of the core board, serving as the visible side of the
exception of Switzerland) Regulation (EU) No. 305/2011 (CPR)
panel after installation, is a layer of solid wood. The surface
applies. The product needs a declaration of performance taking
layer is glued to the core.
into consideration EN 14342:2013, Wood flooring -
Characteristics, evaluation of conformity and marking and the
Backing layer
CE-marking.
The bottom part of the parquet panels is a thin layer of solid
For the application and use the respective national provisions
wood. This layer is added for dimensional stability.
apply.
Glue
2.2 Application
The surface layer and the backing is glued to the substrate with
The multi-layer parquet floorings are intended to be used
low emitting urea-formaldehyde resins.
indoors, in new buildings as well for renovation purposes. The
parquet meets the requirements of EN 13489 and EN 14342.
Finishing
The flooring can be used in residential applications. For
The surface layer is sanded, eventually provided with a bevel
commercial areas conditional use is possible according to the
and finished with UV-curing acrylic lacquers or natural or
manufacturer's instructions.
mineral oils.
2.3 Technical Data The Uniclic/multifit systems are designed to ensure a strong
connection between the Multi-layer parquet flooring elements.
Constructional data
Name Value Unit This product contains substances listed in the Candidate List of
Product minimum thickness 12 mm Substances of Very High Concern for Authorisation REACH
(date: 16.11.2023) exceeding 0.1 percentage by mass: NO
Product maximum thickness 14 mm
Product minimum mass 7,7 kg/m²
This product contains other CMR substances in categories 1A
Product maximum mass 11.8 kg/m² or 1B which are not on the candidate list, exceeding 0.1
Product minimum density 600 kg/m³ percentage by mass: NO
Product maximum density 850 kg/m³
Biocide products were added to this construction product or it
The density of the parquet flooring panels is between 600 and
has been treated with biocide products (this then concerns a
850 kg/m3.
treated product as defined by the (EU) Ordinance on Biocide
Products No. 528/2012): NO
• Performance data of the product in accordance with the
declaration of performance with respect to its essential 2.6 Manufacture
characteristics according to EN 14342:2013 Wood
At the production site in Malaysia core, surface and backing
flooring and parquet — Characteristics, evaluation of
layers are glued together in a hot press. The next step is
conformity and marking and the CE marking.
sawing the planks to lamellas. Then panels are sanded, profiled
• Voluntary data: The product complies with the
(applying the tongue and groove), finished with lacquer or oil,
requirements of the following standard, too EN 13489:
and packed.
Wood Flooring - Multi-layer parquet elements. For the
In production a certified ISO 9001 quality control is in place.
application and use the respective national provisions
apply.
All production machines comply with all regulations in place.
The machines are optimized in respect to energy consumption
2.4 Delivery status
and are equipped with all necessary equipment for safety
Typical standard dimensions are as follows (length - width -
precautions, dust extraction and noise reduction.
thickness)
• 1820mm x 145mm x 14mm 2.7 Environment and health during manufacturing
• 1820mm x 190mm x 14mm The constitutional valid regulations and provisions of the
• 2200mm x 220mm x 14mm national law are observed and respected.
• 2400mm x 260mm x 14mm All coatings and adhesives are water-based solvent free. All
• 580mm x 145mm x 14mm wood waste and cutting and sanding dust is fully heat-recycled.
• 1050mm x 310mm x 14mm Water: There is no wastewater.
• 2200mm x 190mm x 14mm Soil: There is no impact on soil.
• 1820mm x 145mm x 12,5mm Air: The constitutional valid regulations are observed.
2 Environmental Product Declaration - Unilin BV, division flooring - Multi-layer parquet flooring
The emissions to air are far below the legally required comparatively high resistance of the Multilayer parquet flooring,
thresholds. Unilin grants an additional warranty (based on the floor owner
life according to the manufacturer's warranty conditions) for the
In production certified ISO 14001 environmental management declared product. In order to increase the life duration of the
system is in place. floor covering, the manufacturer's instructions concerning
warranty and care must be observed, available for download at
2.8 Product processing/Installation www.unilin.com/en/flooring. The use stage is declared in this
Installation EPD for a one year usage.
The flooring panels are mechanically clicked together without
using glue. The installation can be floating or glued down. In 2.13 Extraordinary effects
case of a floating installation an appropriate underlay must be Fire
used in order to achieve leveling effect, thermal or acoustical In function of the composition of the parquet panel the fire class
insulation and/or protection against rising moisture. The according to EN 13501-1 is Cfl-s1 or Dfl-s1.
following type of underlay materials can be used: The core board is determinative in this respect
• Polyolefin foams • panels are classified as Cfl-s1
• wood fibre panels The fire classification goes for glued down installation and for
• Polyethylene damp proof membranes floating installation on the associated Quick-Step or Pergo
In case of glueing down it is strongly recommended to use underlays.
hybrid elastic mono component-polymer glue which is solvent-
Fire protection
free and water-free.
Name Value
The materials used as underlay or glue are not considered in
this study. Building material class Cfl/Dfl
Appropriate measures for protection against saw dust must be Smoke gas development s1
taken.
Information about the installation of Multilayer parquet flooring
Water
can be downloaded from the website
In case of a floating installation an appropriate DPM (damp
https://www.unilin.com/en/flooring. On this website additional
proof membrane) needs to be installed in order to hold back
technical information (technical data sheets) is available as
potential rising dampness. Most underlays of the Unilin Multi-
well.
layer parquet flooring sales program have a built-in DPM and
2.9 Packaging do not need an extra DPM. The DPM is not a part of this study.
In case of a leak or a flood where the flooring has been soaked
A well-defined number of multilayer parquet flooring panels are
for a longer period of time (days) the flooring will most probably
packed together, putting them with the surface layer onto each
be considered a total loss. In case of short or shorter time of
other. For some of the formats, the packs are edge-protected
exposure and after drying, no visible damage may be expected.
using cardboard and are shrink-wrapped in PE foil. For the
If the water came under the floorcovering (floating installation) it
remaining formats, the panels are packed in a 6-sided
may be necessary to un-click the planks/tiles and let them dry.
cardboard box without shrinkable PE-foil. The packaging
The subfloor will most probably also be wet and should be
materials are fully recyclable.
given the time to come to equilibrium moisture content before
The packs are palletized on wooden pallets using wood from
re-installation of the dry panels. Some of Unilin Multi-layer
controlled origin. The pallets can be re-used (Euro pallets) or
parquet ranges offer a special water resistance and a watertight
recycled as wood category 03 01 05 according to the European
connection between panels. During the installation, the
Waste Catalogue.
periphery needs to be treated with a foam strip and a special
2.10 Condition of use sealant to avoid infiltration. In case of water spillage on the
A thermosetting binding agent and saturating resin are used for surface, it will evaporate before having the chance to penetrate
the production of the flooring panels. When heat and pressure between panels.
are applied during the pressing phase, this is 3D crosslinked by
an irreversible polycondensation reaction. Under normal
conditions, the binding agent and saturating resin are both Mechanical destruction
chemically stable and mechanically firmly bonded to the wood Small(er) damages in the flooring surface can be repaired using
parts. coloured solvent-free melt waxes. In case of more severe
damage the damaged panels can be replaced. The damaged
2.11 Environment and health during use panels go into the normal end-of-life treatment.
All multi-layer parquet floorings of Unilin comply with the health,
2.14 Re-use phase
safety and energy-saving requirements as described in the
harmonised standard EN 14342, type 3. All panels are CE A multi-layer parquet floorcovering which is not at the end-of-life
marked. stage and which is floating, may be un-installed and be re-used
Once the flooring has been installed only very low emissions of as parquet floor.
volatile compounds occur (see chapter 7 of this EPD). These At the end of life stage, the panels can be used as biomass and
emissions originate from the wood. be recycled for example in wood based panels. The panels are
Floorings with a lacquered surface do not need to be re- shredded and reused as raw material in wood-based panels. It
lacquered in domestic use and normal conditions of use. In can also be incinerated in power plants.
case of oiled floors, special periodic maintenance with oilcare
2.15 Disposal
and re-oiling should be done following the manufacturer
Post-installation and post-consumer flooring panels are
maintenance instructions and in function of the intensity of use
considered as wood waste. The European Waste Code EWC is
and the protection in place on the access to outside.
030105. It can be disposed in any regulated municipal waste
2.12 Reference service life collection point as wood waste.
The BBSR Table gives a general useful life of 40 years for floor
coverings of component group 352.812. Due to the
3 Environmental Product Declaration - Unilin BV, division flooring - Multi-layer parquet flooring
DOP (declaration of performance) documents, are available
2.16 Further information either in the packs or can be found on the homepage
All information about the product composition, technical www.unilin.com/en/flooring or can be requested at Unilin BV
performance, instructions for installation and maintenance, division flooring info@unilin.com.
precautionary instructions for use, CE-marking and relevant
3. LCA: Calculation rules
3.1 Declared Unit 3.4 Cut-off criteria
The declared unit is 1 m² of parquet floor covering representing In the assessment, all available data from production process
sales average for both HDF or Hevea core products (average are considered, i.e. all raw materials used, utilised thermal
mass of 9,55 kg/m² and average thickness of 13,25 energy, and electric power consumption using LCI datasets.
mm). Thus material and energy flows contributing less than 1% of
mass or energy are also considered. All reported data are
considered and modelled using LCI data.
Declared unit and mass reference
Name Value Unit
No flows were cut-off that are known to have significant
Declared unit 1 m2 environmental impacts.
Layer thickness 0.01325 m
3.5 Background data
Grammage 9.55 kg/m2
The used background data are from SimaPro version 9
software and the ecoinvent version 3.8 background database.
3.2 System boundary
Type of EPD according to EN 15804: cradle to grave. 3.6 Data quality
The used data refer to the year 2021. The data of the
The production stage includes all relevant processes from foreground processes is based on input-output analyses at the
"cradle to factory gate" within the cut-off rules. This includes for Malaysian production site and Belgian distribution facilities. The
example the extraction and manufacture of all raw materials primary data collection was done thoroughly, all flows were
and their delivery to the production site. The top layer and back considered.
layer material is dried in Europe and then transported to
Malaysia. the manufacturing of the floorcovering panels from 3.7 Period under review
raw material to storage and transport. Packaging is included. The period under review is 2021.
3.8 Geographic Representativeness
The constructional process stage includes the delivery of the
parquet floor covering to the point of installation (A4). The Land or region, in which the declared product system is
transport distance from the plant in Malaysia to the European manufactured, used or handled at the end of the product´s
market via the plant of UNILIN in Wielsbeke and more generally lifespan: Global
the weighted average distance to worldwide market is
considered in this EPD A significant volume is transported
3.9 Allocation
directly to Australia from Malaysia without going through
The overall production of UNILIN comprises further products
Europe. Installation stage (A5) is declared, accounting for
beside the product considered in this study. Data for thermal
electricity consumption, product installation losses, and
and electrical energy as well as auxiliary material refers to the
packaging waste.
declared product. During data collection the allocation is done
via area (m²).
For information on allocation within the background database,
The use stage (B2) includes the cleaning of the parquet for 1
refer to ecoinvent documentation.
year. The cleaning
frequencies are described in chapter 4. Provision of water, 3.10 Comparability
cleaning agent and electricity for the cleaning of the floor
Basically, a comparison or an evaluation of EPD data is only
covering is considered, incl. wastewater treatment.
possible if all the data sets to be compared were created
according to EN 15804 and the building context, respectively
Product end-of-life (C1-C3) comprises the product dismantling,
the product-specific characteristics of performance, are taken
transportation, and energy recovery in combined heat and
into account.
power (CHP) plant. In module C3 the release of biogenic CO2
Background database is as described in chapter 3.5.
is declared according to EN 16485.
Module D includes benefits from all net flows in the end-of-life
stage that leave the product boundary system after having
passed the end-of-waste state. It is assumed that post-
consumer flooring waste is incinerated as waste in a combined
heat and power (CHP) plant. Loads from material incineration
and resulted benefits from recovered energy are declared
within module D.
3.3 Estimates and assumptions
No additional estimates or assumptions had to be made
beyond the information stated in clauses 3 and 4.
4 Environmental Product Declaration - Unilin BV, division flooring - Multi-layer parquet flooring
4. LCA: Scenarios and additional technical information
Maintenance (B2)
Characteristic product properties of biogenic carbon
Maintenance scenario:
Information on describing the biogenic carbon content at
• 1 vacuum cleaning per week
factory gate
• 1 wet cleaning per month (with detergent)
Name ValueUnit
• 1 oil car 3 times per year
kg
Biogenic carbon content in product 4.1 Name Value Unit
C
Water consumption 1.33 kg/m²/year
Biogenic carbon content in accompanying kg
0.24 Detergent 0.0133 kg/m²/year
packaging C
Oil for care 0.0100 kg/m²/year
Note: 1 kg of biogenic carbon is equivalent to 44/12 kg of CO .
2 Electricity consumption (European mix) 0.54 kWh/m²/year
The following technical information is a basis for the declared
modules. Scenarios correspond to the worldwide production Reference service life
and consumption.
Name Value Unit
Reference service life 40 a
Transport to the construction site (A4)
Product shipping stage A4 represents weighted average based End of Life (C1-C4)
on worldwide sales. Name Value Unit
Name Value Unit Collected separately waste type (wood waste) 8.8 kg
Transport distance by boat 12400 km Energy recovery from waste 8.8 kg
Transport distance by truck 875 km
100% of floor covering is incinerated in a combined heat and
Capacity utilisation (including empty runs) for truck 67 % power (CHP) plant.
Installation in the building (A5)
Benefits and loads beyond the product system (D)
Name Value Unit As per IBU PCR Part A, recovered heat is assumed to
Electricity consumption 0.04 kWh substitute to heat generation from natural gas furnace for the
calculation of benefits and loads beyond the product system
Product installation losses 4.0 %
(module D). Produced electricity is assumed to substitute to
Product packaging waste 0.24
grid mix.
5 Environmental Product Declaration - Unilin BV, division flooring - Multi-layer parquet flooring
5. LCA: Results
The LCA results for the MLP-flooring declared in this EPD refer to a MLP-flooring with a thickness of 13.25 mm, which meets the
requirements of EN 14342.
The results for module B2 refer to a period of one year.
DESCRIPTION OF THE SYSTEM BOUNDARY (X = INCLUDED IN LCA; MND = MODULE OR INDICATOR NOT DECLARED; MNR
= MODULE NOT RELEVANT)
Benefits and
Construction loads beyond
Product stage Use stage End of life stage
process stage the system
boundaries
la ire ta m w a Ry lp p u s tro p s n a rT g n iru tc a fu n a M e h t m o rf tro p s n a rTe tis e h t o t e ta g y lb m e s s A e s U e c n a n e tn ia M ria p e R tn e m e c a lp e R tn e m h s ib ru fe R y g re n e la n o ita re p Oe s u re ta w la n o ita re p Oe s u n o itc u rts n o c -e Dn o itilo m e d tro p s n a rT g n is s e c o rp e ts a W la s o p s iD -e s u e R-y re v o c e R-g n ilc y c e Rla itn e to p
A1 A2 A3 A4 A5 B1 B2 B3 B4 B5 B6 B7 C1 C2 C3 C4 D
X X X X X MND X MNR MNR MNR MND MND X X X X X
RESULTS OF THE LCA - ENVIRONMENTAL IMPACT according to EN 15804+A2: 1 m² Multi-layer parquet flooring
Parameter Unit A1 A2 A3 A4 A5 B2 C1 C2 C3 C4 D
GWP-total kg CO 2 eq -1.18E+01 1.16E+00 6.91E+00 2.62E+00 1.73E+00 2.39E-01 0 6.6E-02 1.52E+01 0 -1.11E+01
GWP-fossil kg CO 2 eq 3.31E+00 1.16E+00 7.6E+00 2.61E+00 8.37E-01 2.34E-01 0 6.59E-02 2.14E-01 0 -1.11E+01
GWP-
biogenic kg CO 2 eq -1.52E+01 2.92E-04 -7.39E-01 6.92E-04 8.86E-01 1.29E-03 0 2.14E-05 1.5E+01 0 -8.87E-03
GWP-luluc kg CO 2 eq 1.5E-02 9.29E-04 4.29E-02 1.45E-03 2.45E-03 3.61E-03 0 2.55E-05 1.02E-04 0 -4.19E-03
kg CFC11
ODP 6.29E-06 2.43E-07 4.74E-07 5.71E-07 3.08E-07 1.77E-08 0 1.66E-08 7.3E-09 0 -1.52E-06
eq
AP mol H+ eq 2.46E-02 2.78E-02 3.67E-02 4.26E-02 5.68E-03 1.33E-03 0 2.12E-04 1.3E-02 0 -1.68E-02
EP-
kg P eq 1.76E-04 5.56E-06 3.99E-04 1.46E-05 2.73E-05 2.51E-05 0 4.74E-07 2.68E-05 0 -1.83E-04
freshwater
EP-marine kg N eq 6.23E-03 6.26E-03 5.17E-03 1.03E-02 1.28E-03 2.2E-04 0 4.66E-05 5.75E-03 0 -3.39E-03
EP-terrestrial mol N eq 7.42E-02 6.98E-02 5.64E-02 1.14E-01 1.45E-02 2.03E-03 0 5.18E-04 6.76E-02 0 -3.78E-02
kg NMVOC
POCP 2.31E-02 1.86E-02 1.67E-02 3.08E-02 4.07E-03 5.59E-04 0 2.04E-04 1.56E-02 0 -1.22E-02
eq
ADPE kg Sb eq 4.46E-05 2.18E-06 1.2E-05 6.91E-06 2.91E-06 2.41E-06 0 1.64E-07 3.5E-06 0 -5.54E-06
ADPF MJ 7.4E+01 1.58E+01 8.87E+01 3.71E+01 9.21E+00 4.98E+00 0 1.08E+00 3.42E+00 0 -2E+02
m3 world eq
WDP 4.06E+00 3.83E-02 1.53E+00 9.29E-02 2.38E-01 6.83E-02 0 3.72E-03 5.48E-02 0 -4.53E-01
deprived
GWP = Global warming potential; ODP = Depletion potential of the stratospheric ozone layer; AP = Acidification potential of land and water; EP =
Eutrophication potential; POCP = Formation potential of tropospheric ozone photochemical oxidants; ADPE = Abiotic depletion potential for non-fossil
resources; ADPF = Abiotic depletion potential for fossil resources; WDP = Water (user) deprivation potential)
RESULTS OF THE LCA - INDICATORS TO DESCRIBE RESOURCE USE according to EN 15804+A2: 1 m² Multi-layer parquet
flooring
Parameter Unit A1 A2 A3 A4 A5 B2 C1 C2 C3 C4 D
PERE MJ 5.5E+01 1.42E-01 1.25E+01 4.16E-01 1.57E+01 1.02E+00 0 1.38E-02 1.56E+02 0 -7.26E+00
PERM MJ 1.56E+02 0 6.51E+00 0 -6.38E+00 1.54E-03 0 0 -1.54E+02 0 0
PERT MJ 2.11E+02 1.42E-01 1.91E+01 4.16E-01 9.29E+00 1.02E+00 0 1.38E-02 2.46E+00 0 -7.26E+00
PENRE MJ 5.27E+01 1.58E+01 8.6E+01 3.71E+01 1.2E+01 4.33E+00 0 1.08E+00 2.4E+01 0 -2E+02
PENRM MJ 2.13E+01 0 2.62E+00 0 -2.81E+00 6.37E-01 0 0 -2.06E+01 0 0
PENRT MJ 7.4E+01 1.58E+01 8.87E+01 3.71E+01 9.21E+00 4.97E+00 0 1.08E+00 3.42E+00 0 -2E+02
SM kg 2.61E-04 0 7.17E-02 0 2.88E-03 5.74E-04 0 0 0 0 0
RSF MJ 0 0 0 0 0 0 0 0 0 0 0
NRSF MJ 0 0 0 0 0 0 0 0 0 0 0
FW m3 1.09E-01 1.2E-03 7.26E-02 3.23E-03 8.13E-03 4.31E-03 0 1.26E-04 9.06E-03 0 -3.19E-02
PERE = Use of renewable primary energy excluding renewable primary energy resources used as raw materials; PERM = Use of renewable primary
energy resources used as raw materials; PERT = Total use of renewable primary energy resources; PENRE = Use of non-renewable primary energy
excluding non-renewable primary energy resources used as raw materials; PENRM = Use of non-renewable primary energy resources used as raw
materials; PENRT = Total use of non-renewable primary energy resources; SM = Use of secondary material; RSF = Use of renewable secondary fuels;
NRSF = Use of non-renewable secondary fuels; FW = Use of net fresh water
RESULTS OF THE LCA – WASTE CATEGORIES AND OUTPUT FLOWS according to EN 15804+A2:
1 m² Multi-layer parquet flooring
Parameter Unit A1 A2 A3 A4 A5 B2 C1 C2 C3 C4 D
HWD kg 1.33E-01 1.66E-02 4.1E-01 3.09E-02 3.59E-02 6.23E-03 0 7.48E-04 6.68E-02 0 -5.12E-02
NHWD kg 2.4E+00 4.79E-01 5.74E+00 1.38E+00 4.24E-01 9.36E-02 0 1.07E-01 1.66E-01 0 -5.85E-01
RWD kg 2.84E-04 1.08E-04 6.4E-05 2.54E-04 3.12E-05 3.44E-05 0 7.33E-06 3.61E-05 0 -3.61E-04
CRU kg 0 0 0 0 0 0 0 0 0 0 0
6 Environmental Product Declaration - Unilin BV, division flooring - Multi-layer parquet flooring
MFR kg 9.42E-04 0 7.93E-04 0 6.94E-05 7.44E-04 0 0 0 0 0
MER kg 0 0 0 0 0 0 0 0 0 0 0
EEE MJ 2.31E-01 0 1.88E-01 0 2.04E+00 2.59E-03 0 0 1.4E+01 0 0
EET MJ 4.46E-01 0 3.63E-01 0 3.93E+00 5E-03 0 0 1.35E+02 0 0
HWD = Hazardous waste disposed; NHWD = Non-hazardous waste disposed; RWD = Radioactive waste disposed; CRU = Components for re-use;
MFR = Materials for recycling; MER = Materials for energy recovery; EEE = Exported electrical energy; EET = Exported thermal energy
RESULTS OF THE LCA – additional impact categories according to EN 15804+A2-optional:
1 m² Multi-layer parquet flooring
Parameter Unit A1 A2 A3 A4 A5 B2 C1 C2 C3 C4 D
Disease
PM 6.67E-07 5.65E-08 1.29E-07 1.53E-07 4.4E-08 4.57E-09 0 7.7E-09 2.54E-07 0 -5.21E-08
incidence
IR kBq U235 eq 2.22E-01 6.76E-02 5.16E-02 1.6E-01 2.21E-02 4.15E-02 0 4.69E-03 6.75E-02 0 -3.78E-01
ETP-fw CTUe 2.09E+01 4.82E+00 3.3E+01 1.21E+01 3.25E+00 8.56E-01 0 3.58E-01 5.06E+00 0 -7.42E+00
HTP-c CTUh 2.04E-08 7.37E-10 2.84E-09 1.27E-09 1.3E-09 1.17E-10 0 2.3E-11 2.5E-09 0 -1.33E-09
HTP-nc CTUh 5.81E-08 5.95E-09 5.93E-08 1.81E-08 6.9E-09 3.11E-09 0 7.37E-10 7.1E-08 0 -1.91E-08
SQP SQP 9.99E+02 6.1E+00 7.9E+01 1.73E+01 4.43E+01 1.14E+00 0 1.24E+00 1.01E+00 0 -1.19E+01
PM = Potential incidence of disease due to PM emissions; IR = Potential Human exposure efficiency relative to U235; ETP-fw = Potential comparative
Toxic Unit for ecosystems; HTP-c = Potential comparative Toxic Unit for humans (cancerogenic); HTP-nc = Potential comparative Toxic Unit for humans
(not cancerogenic); SQP = Potential soil quality index
Disclaimer 1 – for the indicator “Potential Human exposure efficiency relative to U235”. This impact category deals mainly with the
eventual impact of low-dose ionizing radiation on human health of the nuclear fuel cycle. It does not consider effects due to possible
nuclear accidents, occupational exposure or radioactive waste disposal in underground facilities. Potential ionizing radiation from the
soil, radon and from some construction materials is also not measured by this indicator.
Disclaimer 2 – for the indicators “abiotic depletion potential for non-fossil resources”, “abiotic depletion potential for fossil resources”,
“water (user) deprivation potential, deprivation-weighted water consumption”, “potential comparative toxic unit for ecosystems”,
“potential comparative toxic unit for humans – cancerogenic”, “Potential comparative toxic unit for humans - not cancerogenic”,
“potential soil quality index”. The results of this environmental impact indicator shall be used with care as the uncertainties on these
results are high as there is limited experience with the indicator.
6. LCA: Interpretation
Benefits and burdens beyond the system boundary (module D)
vary from a few percent to more than 80% of the impacts over
the product life cycle (modules A-C) and relate to the energy
recovery from waste processing in a combined heat and power
plant that is considered to substitute natural gas (heat) and
electricity grid mix.
Figure : Indicator results of multi-layer parquet floor
covering over its life cycle
The largest part of environmental impacts is caused during
production (modules A1-A3) and at waste processing (module
C3); comparably small impacts are caused during the transport
of the product to the construction site.
Maintenance (module B2) is presented for 1 year of product
use, so its impact can be significant over the reference service
life depending on the considered indicator.
All the other modules related to the product life cycle are not
significant.
7 Environmental Product Declaration - Unilin BV, division flooring - Multi-layer parquet flooring
7. Requisite evidence
7.1 PEFC Certificate Wetteren - Belgium. Emission test report of Unilin sample
Engineered wood flooring (new combinations)' nr SPT2021-
The product fulfills the requirements according to PEFC ST R195 from November 9th 2021.
2002:2010: Chain of Custody of Forest Based Products -
• Compliant with AgBB-Scheme 2018 and 2021
Requirements second edition. CTIB - TCHN - Hof ter Vleest
• Compliant with M1 Emission Classification of Building
dreef 3 - 1070 Brussels Belgium
Materials (Testing protocol 15.11.2017)
• Compliant with the French VOC-Regulation: A+
7.2 Formaldehyde emissions
Determination of the formaldehyde emissions of a multi-layer VOC EMISSION RESULTS (AgBB) AFTER 3 days
parquet flooring performed according to the latest versions of Name Value Unit
EN 16516 and ISO 16000 series (part 3, 6 and 9) and to AgBB- TVOC 540 μg/m3
Scheme. – Servaco/Normec Product Testing - Honderweg 13 -
R (dimensionless) 1,427 -
9230 Wetteren - Belgium. Emission test report of Unilin sample
VOC without LCI 21 μg/m3
Engineered wood flooring (new combinations)' nr SPT2021-
R195 from November 9th 2021. Carcinogenic Substances 1 μg/m3
VOC EMISSION RESULTS (AgBB) AFTER 28 days
Name Value Unit
Formaldehyde CAS 50-00-0 24 µg/m3 Name Value Unit
TVOC 280 ug/m3
7.3 VOC emissions
R (dimensionless) 0,376 -
Determination of the VOC emissions of a multi-layer parquet
VOC without LCI 0 ug/m3
flooring performed according to the latest versions of EN 16516
and ISO 16000 series (part 3, 6 and 9) and to AgBB-Scheme. – Carginogenic Substances 0 ug/m3
Servaco/Normec Product Testing - Honderweg 13 - 9230
8. References
Institut Bauen und Umwelt EN 13501-1
Institut Bauen und Umwelt e.V., Berlin (pub.): Fire classification of construction products and building
Generation of Environmental Product Declarations (EPDs); elements, Part 1: Classification using data from reaction to fire
tests, 2007
General principles
for the EPD range of Institut Bauen und Umwelt e.V. (IBU), EN13489:2023
2013-04 www.bau-umwelt.de Wood Flooring - Multi-layer parquet elements.
PCR Part A EN 14342:2013
Institut Bauen und Umwelt e.V., Königswinter (pub.): Wood Flooring - Characteristics, evaluation of conformity and
Product Category Rules for Construction Products from the marking
range of Environmental Product Declarations of Institut Bauen
und Umwelt (IBU), Part A: Calculation Rules for the Life Cycle EN 120 : 1992
Assessment and Requirements on the Background Report. Wood-based panels – Determination of formaldehyde content –
April 2013 www.bau-umwelt.de Extraction method called the perforator method.
ISO 14025:2011-10 EN 717
Environmental labels and declarations — Type III Wood–based panels – Determination of formaldehyde release
environmental declarations — Principles and procedures
ISO 16000-3:2011
ISO 14044: 2006 Indoor air -- Part 3: Determination of formaldehyde and other
Environmental management – Life cycle assessment – carbonyl compounds in indoor air and test chamber air -- Active
Requirements and guidelines (ISO 14044:20) sampling method.
ISO 14040:2006 ISO 16000-6-2011
Environmental management - Life cycle assessment - Indoor air – part 6: Determination of volatile organic compounds
Principles and framework (ISO 14040); German and English in indoor and test chamber air by active sampling on Tenax A
version EN ISO 14040 sorbent, thermal desorption an gas chro-matography using MS
of MS-FID
CEN/TR 15941
Sustainability of construction works - Environmental product ISO 16000-9-2006
declarations - Methodology for selection and use of generic ISO 16000-9:20006 – Indoor air – part 9:
data; German version CEN/TR 15941. Determination of the emissions of volatile organic compounds
from building products and furnishing – Emission test chamber
EN 15804 +A2:2019 method.
Sustainability of construction works — Environmental Product
Declarations — Core rules for the product category of EWC - 94/3/EC Commission Decision of 20 December 1993
construction products. establishing a list of wastes pursuant to Article 1a of Council
Directive 75/442/EEC on waste, 1993 - European Waste
8 Environmental Product Declaration - Unilin BV, division flooring - Multi-layer parquet flooring
Catalogue and Hazardous Waste List Valid from 1 January the Council of the Registration, Evaluation, Authorisation and
2002 Restriction of Chemicals (REACH).
PCR Guidance – Texts for Building-Related Products and ecoinvent
Services – Part B: Requirements on the EPD for floor ecoinvent, Allocation, cut-off by classification, ecoinvent
coverings - IBU Published v6 dated 19.10.2023 database version 3.8 (2021)
PEFC certificate:
Chain of custody ofForest based Product - Requirements - CEN/TR 15941
/PEFC ST 2002:2010. Rapportnumber CTIB-TCHN 0380. Sustainability of construction works - Environmental product
CTIB-TCHN - Hof ter Vleest dreef 3 - 1070 Brussels- Belgium. decla-rations - Methodology for selection and use of generic
data; Ger-man version CEN/TR 15941
REACH
Regulation (EC) No 1907/2006 of the European Parliament and
9 Environmental Product Declaration - Unilin BV, division flooring - Multi-layer parquet flooring
Publisher
Institut Bauen und Umwelt e.V. +49 (0)30 3087748- 0
Hegelplatz 1 info@ibu-epd.com
10117 Berlin www.ibu-epd.com
Germany
Programme holder
Institut Bauen und Umwelt e.V. +49 (0)30 3087748- 0
Hegelplatz 1 info@ibu-epd.com
10117 Berlin www.ibu-epd.com
Germany
Author of the Life Cycle Assessment
EVEA +33 2 28 07 87 00
rue Arthur III, 11 contact@evea-conseil.com
44200 Nantes www.evea-conseil.com/en
France
Owner of the Declaration
Unilin BV, division flooring +32 56 67 52 11
Ooigemstraat 3 info@unilin.com
8710 Wielsbeke www.unilin.com/en/flooring
Belgium
10 Environmental Product Declaration - Unilin BV, division flooring - Multi-layer parquet flooring
