Environmental Product Declaration (EPD)
According to ISO 14025 and EN 15804
Punta PXR
Registration number: EPD-Kiwa-EE-161567-EN
Issue date: 01-03-2024
Valid until: 01-03-2029
Declaration owner: Ansorg GmbH
Publisher: Kiwa-Ecobility Experts
Program operator: Kiwa-Ecobility Experts
Status: verified
Punta PXR | ReTHiNK-61567 1 / 19
Environmental Product Declaration
1 General information
Production location:Ansorg GmbH
1.1 PRODUCT Address production location:Pilgerstraße 11, 45473 Mülheim an der Ruhr, Germany
Punta PXR
1.6 VERIFICATION OF THE DECLARATION
1.2 REGISTRATION NUMBER
The independent verification is in accordance with the ISO 14025:2011. The LCA is in
EPD-Kiwa-EE-161567-EN compliance with ISO 14040:2006 and ISO 14044:2006. The EN 15804:2012+A2:2019 serves as
the core PCR.
1.3 VALIDITY Internal External
Issue date:01-03-2024
Valid until:01-03-2029
1.4 PROGRAM OPERATOR
Kiwa-Ecobility Experts
Wattstraße 11-13
13355 Berlin Elisabeth Amat Guasch, Greenize
DE
1.7 STATEMENTS
The owner of this EPD shall be liable for the underlying information and evidence. The
programme operator Kiwa-Ecobility Experts shall not be liable with respect to
manufacturer data, life cycle assessment data and evidence.
Raoul Mancke Dr. Ronny Stadie
1.8 PRODUCT CATEGORY RULES
(Head of programme operations, Kiwa- (Verification body, Kiwa-Ecobility Experts)
Ecobility Experts) PCR A: Kiwa-Ecobility Experts (Kiwa-EE) – General Product Category Rules (2022-02-14)
PCR B: Institute Construction and Environment e.V. (IBU) - Part B: Requirements on the
1.5 OWNER OF THE DECLARATION EPD for Luminaires, lamps and components for luminaires
Manufacturer:Ansorg GmbH
1.9 COMPARABILITY
Address:Pilgerstraße 11, 45473 Mülheim an der Ruhr, Germany
E-mail:info@ansorg.com In principle, a comparison or assessment of the environmental impacts of different
products is only possible if they have been prepared in accordance with EN 15804. For the
Website:www.ansorg.com evaluation of the comparability, the following aspects have to be considered in particular:
PCR used, functional or declared unit, geographical reference, the definition of the system
Punta PXR | ReTHiNK-61567 2 / 19
Environmental Product Declaration
1 General information
boundary, declared modules, data selection (primary or secondary data, background Characterization method:EN 15804 +A2 Method v1.0
database, data quality), scenarios used for use and disposal phases, and the life cycle
inventory (data collection, calculation methods, allocations, validity period). PCRs and LCA database profiles:EcoInvent version 3.6
general program instructions of different EPDs programs may differ. Comparability needs Version database:v3.16 (2024-02-12)
to be evaluated. For further guidance, see EN 15804+A2 (5.3 Comparability of EPD for
construction products) and ISO 14025 (6.7.2 Requirements for comparability). *Used for calculating the characterized results of the Environmental profiles within
R<THiNK.
1.10 CALCULATION BASIS
1.11 LCA BACKGROUND REPORT
LCA method R<THiNK:Ecobility Experts | EN15804+A2
This EPD is generated on the basis of the LCA background report 'Punta PXR' with the
LCA software*:Simapro 9.1
calculation identifier ReTHiNK-61567.
Punta PXR | ReTHiNK-61567 3 / 19
Environmental Product Declaration
2 Product
2.1 PRODUCT DESCRIPTION • Return of light – significant reduction of connected load through targeted light
guidance
Punta is a luminaire for versatile applications, from precise spot effects to the illumination
Data sheets and further information about the Punta PXR can be found on the product
of peripheral zones and high decorations. The housing is flexibly positioned on a ring
pages of our website www.ansorg.com.
bearing to permit maximum rotation. It pivots smoothly and alignment is easily
maintained without locking. A large pivot radius provides plenty of flexibility for adaptation
to shop design changes. The reflector technology employed ensures very efficient and
brilliant light distribution.
• The Punta PXR delivers a maximum power level of 16W. With a light quality of
3000K and CRI 80, for example, it can achieve a luminous flux of 1780 lumens. The
Punta PXR is thus the most powerful recessed spotlight in terms of size.
• Compared to the previous version (Punta NRL), efficiency has been boosted by over
40% (NRL 85lm/W vs. PXR 123lm/W with a colour temperature of warm white [830]).
• The smallest Ansorg 3D faceted reflector. The smallest Punta therefore now also
has the superior lighting quality (light blending, glare suppression and high ROL)
of the larger luminaires in the Punta family.
• The luminaire can be rotated by 355° and has a swing-out angle of 0°–45°.
The Punta PXR consists mainly of the following materials:
• Aluminium (46%)
• Electronic connector (26%)
• Cables (14%)
• Steel (10%)
• Plastics (1%)
Punta PXR facts
• LED technology
• Tool-free in-ceiling installation
• Floor and wall mounting not admissible
• Rotates and pivots (355°/45°)
• Including SP, MFL or FL reflector
• Including power module
• Main connection via Wieland plug GST18i3; cable length = 0.5 m
• DALI or Casambi lighting control system on request
• Colours: white, anthracite, silver
Punta PXR sustainability
• Completely sustainable packaging
• 100% recyclable luminaire in accordance with the WEEE Directive (Directive
2012/19/EU on waste electrical and electronic equipment)
• Designed in accordance with the Ecodesign Regulation (2019/2020/EU)
• High LED lifespan through efficient thermal management
Punta PXR | ReTHiNK-61567 4 / 19
Environmental Product Declaration
2 Product
2.2 APPLICATION (INTENDED USE OF THE PRODUCT) 2.5 SUBSTANCES OF VERY HIGH CONCERN
Applications: For open ceilings. From accentuated lighting to the illumination of large The product does not contain any substances from the candidate list of substances of very
areas. Various power levels and colour temperatures, e.g. for back wall illumination or high concern for authorisation (SVHC). The suppliers and Ansorg GmbH comply with the
highlight zones. legal requirements according to REACH Directive (EU) 2023/1132 and ROHS Directive
2015/863 and 2023/1437.
Sectors: All sectors.
The designated products also comply with the ISO 9001 and ISO 14001 standards, and with
Efficient substitute for low-voltage halogen reflector lamps. Use of different colour the EcoVadis Silver Medal and the SMETA 2-Pillar certifications.
temperatures possible. Cold white to warm white with different colour rendering levels
and excellent efficiency.
2.6 DESCRIPTION PRODUCTION PROCESS
2.3 REFERENCE SERVICE LIFE
The individual materials are delivered to Ansorg and assembled at the production site. It is
RSL PRODUCT internally transported, packaged and stored by Ansorg. They are then brought to a
distribution centre, from where it is transported to the customer.
The Reference Service Life (RSL) has been calculated based on the amount of hours that
the light can be used (66,000 hours). It is assumed that the light is used for 12 hours a day,
for 6 days a week (excluding Sunday because the majority of companies in the retail and
service sector are closed then), for 52 weeks a year. Therefore, 66,000 is divided by (6*12)
and 52, which leads to a number of approximately 17.
USED RSL (YR) IN THIS LCA CALCULATION:
17
2.4 TECHNICAL DATA
• Connection data 220–240 V, 50/60 Hz (110–277 V on request)
• Weight approx. 0.4 kg
• SDCM rating 3SDCM (MacAdam)
• Lumen maintenance L80/B10 ≥ 50,000 h, TA 25 °C
L90/B50 ≥ 50,000 h, TA 25 °C
• Failure rate C0/B10 ≥ 50,000 h, TA 25 °C
• Photobiological safety RG1
• Number per circuit breaker B 16A 34
• Protection class 1
• Type of protection IP20
• Certification mark ENEC / EB
2.7 CONSTRUCTION DESCRIPTION
This product can be mounted on a surface without tools.
Punta PXR | ReTHiNK-61567 5 / 19
Environmental Product Declaration
3 Calculation rules
3.1 FUNCTIONAL UNIT 3.3 SCOPE OF DECLARATION AND SYSTEM BOUNDARIES
1 piece lighting This is a Cradle to gate with options, modules C1-C4 and module D LCA. The life cycle
Provides lighting that delivers various artificial luminous fluxes during a reference lifetime stages included are as shown below:
of 66,000 hours.
(X = module included, ND = module not declared)
reference_unit: piece (p) A1 A2 A3 A4 A5 B1 B2 B3 B4 B5 B6 B7 C1 C2 C3 C4 D
X X X X X X ND ND ND ND X ND X X X X X
3.2 CONVERSION FACTORS
The modules of the EN15804 contain the following:
Description Value Unit
reference_unit 1 p Module A1 = Raw material supply Module B5 = Refurbishment
weight_per_reference_unit 0.408 kg Module A2 = Transport Module B6 = Operational energy use
Conversion factor to 1 kg 2.453386 p Module A3 = Manufacturing Module B7 = Operational water use
Module A4 = Transport Module C1 = De-construction / Demolition
Module A5 = Construction -
Module C2 = Transport
Installation process
Module B1 = Use Module C3 = Waste Processing
Module B2 = Maintenance Module C4 = Disposal
Module D = Benefits and loads beyond the
Module B3 = Repair
product system boundaries
Module B4 = Replacement
3.4 REPRESENTATIVENESS
The input data are representative for Lights, a product of Ansorg GmbH. The data are
representative for Germany.
3.5 CUT-OFF CRITERIA
Production phase (Modules A1-A3)
All input flows (e.g. raw materials, transportation, energy use, packaging, etc.) and output
flows (e.g. production waste) are considered in this LCA. The internal transport of the
products is not considered, because it falls under the cut-off criteria. The total neglected
input flows do not exceed the limit of 5% of energy use and mass.
Punta PXR | ReTHiNK-61567 6 / 19
Environmental Product Declaration
3 Calculation rules
Construction phase (Modules A4-A5) 3.8 ESTIMATES AND ASSUMPTIONS
All input flows (e.g. transportation to the construction site, additional raw material use for For data protection reasons, various assumptions made on the data used for this EPD are
construction, installation energy, energy use for assembly, etc.) and output flows (e.g. only explained in the background report accompanying this EPD.
construction waste, packaging waste, etc.), if applicable, are considered in this LCA. The
total neglected input flows do not exceed the limit of 5% of energy use and mass. For module A4, a capacity utilization of 90% has been taken to reflect reality.
Delivery of the luminaire throughout Europe is considered. Of the use phase, only module B6 (Operational Energy Use) is declared. The numbers for
this are calculated based on the formula given in the PCR. According to the PCR, the
operational energy use should be calculated based on the type of product (luminaire,
Use phase (Module B6) lamp, or lamp component). This product is a luminaire. The energy consumption of a
luminaire can be calculated with the following formula:
For the use phase, the input and output flows for Module B6 (operational energy use) are
considered in this LCA. The total neglected input flows do not exceed the limit of 5% of Energy consumption [kWh] = {Pa * FCP * FO * ( FD * tD + FN * tN) + Pp * ty} * 1/1000 * a
energy use and mass.
• Pa [W] = active power
• FCP = product constant illuminance factor
End-of-Life phase (Modules C1-C4) • FO = occupancy dependency factor
• FD = daylight dependency factor
All input flows (e.g. energy use for demolition or disassembly, transport to waste
• tD [h] = daylight operating hours per year
processing, etc.) and output flows (e.g. end-of-life waste processing of the product, etc.) are
• FN = non-daylight dimming factor
considered in this LCA. The total neglected input flows do not exceed the limit of 5% of
• tN [h] = non-daylight operating hours per year
energy use and mass.
• Pp [W] = passive power
• ty [h] = 8760
Benefits and loads beyond the system boundary (Module D) • a = reference service lifetime of installation in years
All benefits and loads beyond the system boundary resulting from reusable products, The exact calculation for this product is given in the corresponding background report. For
recyclable materials and/or useful energy carriers leaving the product system are some parameters an assumption had to be made, because no information on it is
considered in this LCA. available. Therefore, the numbers for B6 are conservative numbers.
The emissions calculated for module B6 are for the full reference service lifetime of 66,000
3.6 ALLOCATION hours or approximately 17 years.
Allocation has not been applied in this LCA.
3.9 DATA QUALITY
3.7 DATA COLLECTION & REFERENCE TIME PERIOD The quality of the data is high.
In order to ensure comparability of the results, only consistent background data of the
All product- and process-specific data were collected for the operating years 2021 and
Ecoinvent database V3.6 was used in the LCA (e.g., records on energy, transportation,
2022. The data is based on the exact figures of this year.
supplies and supplies), which refers to reference year 2019. The database is regularly
reviewed and thus complies with the requirements of EN 15804 (background data not
older than 10 years). All consistent datasets contained in the Ecoinvent database are
documented and can be viewed in the online Ecoinvent documentation. The primary data
were provided by Ansorg. The life cycle was modelled with the Nibe EPD App.
Punta PXR | ReTHiNK-61567 7 / 19
Environmental Product Declaration
4 Scenarios and additional technical information
4.1 TRANSPORT TO CONSTRUCTION SITE (A4)
For the transport from production place to assembly/user, the following scenario is
assumed for module A4 of this EPD.
Value and unit
Vehicle type used for transport Lorry (Truck), unspecified (default) | market group for (GLO)
Fuel type and consumption of vehicle
Distance 1051 km
Capacity utilisation (including empty returns) 90%
Bulk density of transported products
Volume capacity utilisation factor
4.2 ASSEMBLY (A5)
The following information describes the scenarios for flows entering the system and flows
leaving the system at module A5.
FLOWS ENTERING THE SYSTEM
There are no significant environment impacts as a result of materials or energy used in the
construction stage (A5).
FLOWS LEAVING THE SYSTEM
The following output flows leaving the system at module A5 are assumed.
Description Value Unit
Output materials as result of loss during construction 0 %
Output materials as result of waste processing of materials used for installation/assembly at the building site 0.000 kg
Output materials as result of waste processing of used packaging 0.230 kg
4.3 USE STAGE (B6)
Emissions to air/soil/water are applicable, the scenario accounted in module B6 is as
follows:
Description Cycle (yr) Number of cycles Amount per cycle Total Amount Unit
Use phase electricity 17 1 705.5 705.5 kWh
Punta PXR | ReTHiNK-61567 8 / 19
Environmental Product Declaration
4 Scenarios and additional technical information
4.4 DE-CONSTRUCTION, DEMOLITION (C1)
No inputs are needed for the product at the de-construction / demolition phase
4.5 TRANSPORT END-OF-LIFE (C2)
The following distances and transport conveyance are assumed for transportation during
end of life for the different types of waste processing.
Waste Scenario Transport conveyance Not removed (stays in Landfill Incineration Recycling Re-use
work) [km] [km] [km] [km] [km]
aluminium, cast alloy for buildings (i.a. profiles, Lorry (Truck), unspecified (default) | market
0 100 150 50 0
sheets, pipes) (NMD ID 4) group for (GLO)
Lorry (Truck), unspecified (default) | market
finishes (adhered to wood, plastic, metal) (NMD ID 2) 0 100 150 50 0
group for (GLO)
Lorry (Truck), unspecified (default) | market
Galvanised steel (i.a. profiles, sheets) (NMD ID 75) 0 100 150 50 0
group for (GLO)
Lorry (Truck), unspecified (default) | market
plastics, via residue (NMD ID 43) 0 100 150 50 0
group for (GLO)
Lorry (Truck), unspecified (default) | market
EoL electronics - passive components 0 100 150 50 0
group for (GLO)
Lorry (Truck), unspecified (default) | market
PVC, pipes (NMD ID 64) 0 100 150 50 0
group for (GLO)
The transport conveyance(s) used in the scenario(s) for transport during end of life has the
following characteristics.
Value and unit
Vehicle type used for transport Lorry (Truck), unspecified (default) | market group for (GLO)
Fuel type and consumption of vehicle not available
Capacity utilisation (including empty returns) 50 % (loaded up and return empty)
Bulk density of transported products inapplicable
Volume capacity utilisation factor 1
Punta PXR | ReTHiNK-61567 9 / 19
Environmental Product Declaration
4 Scenarios and additional technical information
4.6 END OF LIFE (C3, C4)
The scenario(s) assumed for end of life of the product are given in the following tables.
First the assumed percentages per type of waste processing are displayed, followed by the
assumed amounts.
Waste Scenario Region Not removed (stays in work) [%] Landfill [%] Incineration [%] Recycling [%] Re-use [%]
aluminium, cast alloy for buildings (i.a. profiles, sheets, pipes) (NMD ID 4) NL 0 3 3 94 0
finishes (adhered to wood, plastic, metal) (NMD ID 2) NL 0 0 100 0 0
Galvanised steel (i.a. profiles, sheets) (NMD ID 75) NL 0 5 0 95 0
plastics, via residue (NMD ID 43) NL 0 20 80 0 0
EoL electronics - passive components DE 0 5 35 60 0
PVC, pipes (NMD ID 64) NL 0 10 20 70 0
Waste Scenario Not removed (stays in work) [kg] Landfill [kg] Incineration [kg] Recycling [kg] Re-use [kg]
aluminium, cast alloy for buildings (i.a. profiles, sheets, pipes) (NMD ID 4) 0.000 0.006 0.006 0.176 0.000
finishes (adhered to wood, plastic, metal) (NMD ID 2) 0.000 0.000 0.004 0.000 0.000
Galvanised steel (i.a. profiles, sheets) (NMD ID 75) 0.000 0.002 0.000 0.038 0.000
plastics, via residue (NMD ID 43) 0.000 0.002 0.009 0.000 0.000
EoL electronics - passive components 0.000 0.007 0.050 0.085 0.000
PVC, pipes (NMD ID 64) 0.000 0.002 0.005 0.017 0.000
Total 0.000 0.019 0.073 0.315 0.000
4.7 BENEFITS AND LOADS BEYOND THE SYSTEM BOUNDARY (D)
The presented Benefits and loads beyond the system boundary in this EPD are based on
the following calculated Net output flows in kilograms and Energy recovery displayed in
MJ Lower Heating Value.
Waste Scenario Net output flow [kg] Energy recovery [MJ]
aluminium, cast alloy for buildings (i.a. profiles, sheets, pipes) (NMD ID 4) 0.176 0.000
finishes (adhered to wood, plastic, metal) (NMD ID 2) 0.000 0.000
Total 0.315 0.160
Punta PXR | ReTHiNK-61567 10 / 19
Environmental Product Declaration
4 Scenarios and additional technical information
Waste Scenario Net output flow [kg] Energy recovery [MJ]
Galvanised steel (i.a. profiles, sheets) (NMD ID 75) 0.038 0.000
plastics, via residue (NMD ID 43) 0.000 0.160
EoL electronics - passive components 0.085 0.000
PVC, pipes (NMD ID 64) 0.017 0.000
Total 0.315 0.160
Punta PXR | ReTHiNK-61567 11 / 19
Environmental Product Declaration
5 Results
For the impact assessment, the characterization factors of the LCIA method EN 15804 +A2
Method v1.0 are used. Long-term emissions (>100 years) are not considered in the impact
assessment. The results of the impact assessment are only relative statements that do not
make any statements about end-points of the impact categories, exceedance of threshold
values, safety margins or risks. The following tables show the results of the indicators of the
impact assessment, of the use of resources as well as of waste and other output flows.
5.1 ENVIRONMENTAL IMPACT INDICATORS PER PIECE
CORE ENVIRONMENTAL IMPACT INDICATORS EN15804+A2
Abbreviation Unit A1 A2 A3 A4 A5 B6 C1 C2 C3 C4 D
AP mol H+ eqv. 8.96E-2 1.57E-3 1.29E-3 5.24E-4 8.12E-5 1.77E+0 0.00E+0 2.24E-5 3.28E-4 2.77E-6 -2.07E-2
GWP-total kg CO2 eqv. 6.76E+0 6.61E-2 -1.70E-1 9.05E-2 3.91E-1 3.13E+2 0.00E+0 3.87E-3 2.24E-1 1.71E-3 -2.82E+0
GWP-b kg CO2 eqv. -1.34E-2 -3.37E-6 -3.74E-1 4.17E-5 3.76E-1 9.09E+0 0.00E+0 1.78E-6 -7.53E-5 5.02E-6 3.78E-1
GWP-f kg CO2 eqv. 6.75E+0 6.60E-2 2.02E-1 9.04E-2 1.56E-2 3.03E+2 0.00E+0 3.86E-3 2.24E-1 1.71E-3 -3.19E+0
GWP-luluc kg CO2 eqv. 2.84E-2 3.86E-5 2.62E-3 3.31E-5 4.66E-6 7.04E-1 0.00E+0 1.42E-6 4.45E-5 2.77E-7 -1.22E-2
EP-m kg N eqv. 8.52E-3 3.98E-4 3.17E-4 1.85E-4 2.89E-5 2.24E-1 0.00E+0 7.90E-6 6.94E-5 2.74E-6 -3.11E-3
EP-fw kg P eqv. 6.84E-4 4.01E-7 1.96E-5 9.12E-7 2.26E-7 3.23E-2 0.00E+0 3.90E-8 2.11E-6 1.11E-8 -1.05E-4
EP-T mol N eqv. 1.04E-1 4.43E-3 3.69E-3 2.04E-3 3.08E-4 2.76E+0 0.00E+0 8.71E-5 7.80E-4 8.68E-6 -3.44E-2
kg CFC 11
ODP 3.49E-7 1.37E-8 2.32E-8 2.00E-8 2.30E-9 2.55E-5 0.00E+0 8.53E-10 7.04E-9 7.04E-11 -1.29E-7
eqv.
kg NMVOC
POCP 2.93E-2 1.16E-3 9.28E-4 5.82E-4 1.03E-4 7.01E-1 0.00E+0 2.49E-5 2.13E-4 2.82E-6 -1.04E-2
eqv.
ADP-f MJ 7.28E+1 8.94E-1 3.20E+0 1.36E+0 1.72E-1 6.23E+3 0.00E+0 5.83E-2 5.85E-1 6.59E-3 -3.03E+1
ADP-mm kg Sb-eqv. 4.74E-4 8.80E-7 1.40E-6 2.29E-6 4.79E-7 2.20E-3 0.00E+0 9.79E-8 1.26E-6 3.23E-9 7.04E-4
m3 world
WDP 1.78E+0 2.00E-3 7.86E-2 4.88E-3 9.47E-4 6.98E+1 0.00E+0 2.09E-4 1.16E-2 2.10E-4 -3.03E-1
eqv.
AP=Acidification (AP) | GWP-total=Global warming potential (GWP-total) | GWP-b=Global warming potential - Biogenic (GWP-b) | GWP-f=Global warming potential - Fossil (GWP-f) | GWP-
luluc=Global warming potential - Land use and land use change (GWP-luluc) | EP-m=Eutrophication marine (EP-m) | EP-fw=Eutrophication, freshwater (EP-fw) | EP-T=Eutrophication,
terrestrial (EP-T) | ODP=Ozone depletion (ODP) | POCP=Photochemical ozone formation - human health (POCP) | ADP-f=Resource use, fossils (ADP-f) | ADP-mm=Resource use, minerals and
metals (ADP-mm) | WDP=Water use (WDP)
Punta PXR | ReTHiNK-61567 12 / 19
Environmental Product Declaration
5 Results
ADDITIONAL ENVIRONMENTAL IMPACT INDICATORS EN15084+A2
Abbreviation Unit A1 A2 A3 A4 A5 B6 C1 C2 C3 C4 D
ETP-fw CTUe 6.73E+2 6.57E-1 9.23E+0 1.22E+0 2.85E-1 4.27E+3 0.00E+0 5.20E-2 3.14E+0 3.50E+0 -7.52E+1
disease
PM 5.37E-7 3.32E-9 1.65E-8 8.14E-9 1.49E-9 4.63E-6 0.00E+0 3.48E-10 3.64E-9 4.43E-11 -2.49E-7
incidence
HTP-c CTUh 1.75E-8 3.46E-11 2.32E-10 3.94E-11 1.19E-11 1.10E-7 0.00E+0 1.69E-12 7.36E-11 3.30E-13 -4.35E-9
HTP-nc CTUh 7.33E-7 6.11E-10 3.29E-9 1.33E-9 2.08E-10 3.76E-6 0.00E+0 5.69E-11 4.72E-9 1.29E-11 -6.16E-8
IR kBq U235 eqv. 1.71E-1 3.80E-3 1.43E-2 5.71E-3 7.80E-4 5.39E+1 0.00E+0 2.44E-4 2.37E-3 2.47E-5 -4.00E-2
SQP Pt 2.74E+1 3.61E-1 3.69E+1 1.18E+0 6.92E-2 1.52E+3 0.00E+0 5.06E-2 4.74E-1 1.21E-2 -1.99E+1
ETP-fw=Ecotoxicity, freshwater (ETP-fw) | PM=Particulate Matter (PM) | HTP-c=Human toxicity, cancer (HTP-c) | HTP-nc=Human toxicity, non-cancer (HTP-nc) | IR=Ionising radiation, human
health (IR) | SQP=Land use (SQP)
CLASSIFICATION OF DISCLAIMERS TO THE DECLARATION OF CORE AND ADDITIONAL ENVIRONMENTAL IMPACT INDICATORS
ILCD classification Indicator Disclaimer
Global warming potential (GWP) None
ILCD type / level 1 Depletion potential of the stratospheric ozone layer (ODP) None
Potential incidence of disease due to PM emissions (PM) None
AAcidification potential, Accumulated Exceedance (AP) None
Eutrophication potential, Fraction of nutrients reaching freshwater end compartment
None
(EP-freshwater)
Eutrophication potential, Fraction of nutrients reaching marine end compartment
ILCD type / level 2 None
(EP-marine)
Eutrophication potential, Accumulated Exceedance (EP-terrestrial) None
Formation potential of tropospheric ozone (POCP) None
Potential Human exposure efficiency relative to U235 (IRP) 1
Abiotic depletion potential for non-fossil resources (ADP-minerals&metals) 2
ILCD type / level 3
Abiotic depletion potential for fossil resources (ADP-fossil) 2
Water (user) deprivation potential, deprivation-weighted water consumption (WDP) 2
Potential Comparative Toxic Unit for ecosystems (ETP-fw) 2
Punta PXR | ReTHiNK-61567 13 / 19
Environmental Product Declaration
5 Results
ILCD classification Indicator Disclaimer
Potential Comparative Toxic Unit for humans (HTP-c) 2
Potential Comparative Toxic Unit for humans (HTP-nc) 2
Potential Soil quality index (SQP) 2
Disclaimer 1 – This impact category deals mainly with the eventual impact of low dose ionizing radiation on human health of the nuclear fuel cycle. It does not consider effects due to possible
nuclear accidents, occupational exposure nor due to radioactive waste disposal in underground facilities. Potential ionizing radiation from the soil, from radon and from some construction
materials is also not measured by this indicator.
Disclaimer 2 – The results of this environmental impact indicator shall be used with care as the uncertainties on these results are high or as there is limited experienced with the indicator.
5.2 INDICATORS DESCRIBING RESOURCE USE AND ENVIRONMENTAL INFORMATION BASED ON LIFE CYCLE INVENTORY (LCI)
PARAMETERS DESCRIBING RESOURCE USE
Abbreviation Unit A1 A2 A3 A4 A5 B6 C1 C2 C3 C4 D
PERE MJ 9.90E+0 7.92E-3 4.21E+0 1.71E-2 5.80E-3 1.18E+3 0.00E+0 7.30E-4 5.21E-2 2.34E-4 -3.65E+0
PERM MJ 0.00E+0 0.00E+0 3.59E+0 0.00E+0 0.00E+0 0.00E+0 0.00E+0 0.00E+0 0.00E+0 0.00E+0 -2.79E+0
PERT MJ 9.90E+0 7.92E-3 7.80E+0 1.71E-2 5.80E-3 1.18E+3 0.00E+0 7.30E-4 5.95E-2 2.67E-4 -6.44E+0
PENRE MJ 7.74E+1 9.49E-1 3.33E+0 1.45E+0 1.82E-1 6.54E+3 0.00E+0 6.19E-2 5.41E-1 5.12E-3 -3.19E+1
PENRM MJ 2.00E-1 0.00E+0 7.32E-2 0.00E+0 0.00E+0 0.00E+0 0.00E+0 0.00E+0 0.00E+0 0.00E+0 -2.42E-1
PENRT MJ 7.76E+1 9.49E-1 3.41E+0 1.45E+0 1.82E-1 6.54E+3 0.00E+0 6.19E-2 6.25E-1 7.01E-3 -3.21E+1
SM Kg 0.00E+0 0.00E+0 0.00E+0 0.00E+0 0.00E+0 0.00E+0 0.00E+0 0.00E+0 0.00E+0 0.00E+0 0.00E+0
RSF MJ 0.00E+0 0.00E+0 0.00E+0 0.00E+0 0.00E+0 0.00E+0 0.00E+0 0.00E+0 0.00E+0 0.00E+0 0.00E+0
NRSF MJ 0.00E+0 0.00E+0 0.00E+0 0.00E+0 0.00E+0 0.00E+0 0.00E+0 0.00E+0 0.00E+0 0.00E+0 0.00E+0
FW M3 6.27E-2 6.94E-5 2.69E-3 1.66E-4 3.97E-5 5.21E+0 0.00E+0 7.10E-6 4.52E-4 6.07E-6 -1.81E-2
PERE=renewable primary energy ex. raw materials | PERM=renewable primary energy used as raw materials | PERT=renewable primary energy total | PENRE=non-renewable primary energy
ex. raw materials | PENRM=non-renewable primary energy used as raw materials | PENRT=non-renewable primary energy total | SM=use of secondary material | RSF=use of renewable
secondary fuels | NRSF=use of non-renewable secondary fuels | FW=use of net fresh water
Punta PXR | ReTHiNK-61567 14 / 19
Environmental Product Declaration
5 Results
OTHER ENVIRONMENTAL INFORMATION DESCRIBING WASTE CATEGORIES
Abbreviation Unit A1 A2 A3 A4 A5 B6 C1 C2 C3 C4 D
HWD Kg 1.05E-3 1.35E-6 6.78E-6 3.46E-6 4.89E-7 4.15E-3 0.00E+0 1.48E-7 1.16E-3 8.29E-9 1.41E-3
NHWD Kg 1.50E+0 2.21E-2 3.50E-2 8.65E-2 4.94E-3 2.11E+1 0.00E+0 3.70E-3 2.09E-2 1.95E-2 -6.01E-1
RWD Kg 1.53E-4 6.09E-6 1.55E-5 8.96E-6 1.11E-6 4.42E-2 0.00E+0 3.83E-7 2.50E-6 3.33E-8 -4.69E-5
HWD=hazardous waste disposed | NHWD=non hazardous waste disposed | RWD=radioactive waste disposed
ENVIRONMENTAL INFORMATION DESCRIBING OUTPUT FLOWS
Abbreviation Unit A1 A2 A3 A4 A5 B6 C1 C2 C3 C4 D
CRU Kg 0.00E+0 0.00E+0 0.00E+0 0.00E+0 0.00E+0 0.00E+0 0.00E+0 0.00E+0 0.00E+0 0.00E+0 0.00E+0
MFR Kg 0.00E+0 0.00E+0 0.00E+0 0.00E+0 2.30E-1 0.00E+0 0.00E+0 0.00E+0 2.30E-1 0.00E+0 0.00E+0
MER Kg 0.00E+0 0.00E+0 0.00E+0 0.00E+0 0.00E+0 0.00E+0 0.00E+0 0.00E+0 0.00E+0 0.00E+0 0.00E+0
EET MJ 0.00E+0 0.00E+0 0.00E+0 0.00E+0 0.00E+0 0.00E+0 0.00E+0 0.00E+0 0.00E+0 0.00E+0 4.96E-2
EEE MJ 0.00E+0 0.00E+0 0.00E+0 0.00E+0 0.00E+0 0.00E+0 0.00E+0 0.00E+0 0.00E+0 0.00E+0 2.88E-2
CRU=Components for re-use | MFR=Materials for recycling | MER=Materials for energy recovery | EET=Exported Energy Thermic | EEE=Exported Energy Electric
Punta PXR | ReTHiNK-61567 15 / 19
Environmental Product Declaration
5 Results
5.3 INFORMATION ON BIOGENIC CARBON CONTENT PER PIECE
BIOGENIC CARBON CONTENT
The following Information describes the biogenic carbon content in (the main parts of) the
product at the factory gate per piece:
Biogenic carbon content Amount Unit
Biogenic carbon content in the product 0 kg C
Biogenic carbon content in accompanying packaging 0.1025 kg C
UPTAKE OF BIOGENIC CARBON DIOXIDE
The following amount of uptake of carbon dioxide is account in module A1 by the main
parts of the product. Related uptake and release of carbon dioxide in downstream
processes are not taken into account in this number although they do appear in the
presented results.
Uptake Biogenic Carbon dioxide Amount Unit
Packaging 0.3757 kg CO2 (biogenic)
Punta PXR | ReTHiNK-61567 16 / 19
Environmental Product Declaration
6 Interpretation of results
As can be seen in the graph, Module B6 (Operational energy use) has the biggest influence
in all environmental impact categories. After that, Module A1 (Raw material preparation)
has the biggest influence in most of the categories. In the category Resource use -
minerals and metals (ADP-mm), Module D (Benefits and loads beyond the system
boundary) has the biggest influence after Module B6.
Punta PXR | ReTHiNK-61567 17 / 19
Environmental Product Declaration
7 References
ISO 14040
ISO 14040:2006-10, Environmental management - Life cycle assessment - Principles and
framework; EN ISO 14040:2006
ISO 14044
ISO 14044:2006-10, Environmental management - Life cycle assessment - Requirements
and guidelines; EN ISO 14040:2006
ISO 14025
ISO 14025:2011-10: Environmental labels and declarations — Type III environmental
declarations — Principles and procedures
EN 15804+A2
EN 15804+A2: 2019: Sustainability of construction works — Environmental Product
Declarations — Core rules for the product category of construction products
PCR B
Institute Construction and Environment e.V. (IBU) - Part B: Requirements on the EPD for
Luminaires, lamps and components for luminaires
Punta PXR | ReTHiNK-61567 18 / 19
Environmental Product Declaration
8 Contact information
Publisher Operator Owner of declaration
Kiwa-Ecobility Experts Kiwa-Ecobility Experts Ansorg GmbH
Wattstraße 11-13 Wattstraße 11-13 Pilgerstraße 11
13355 Berlin, DE 13355 Berlin, DE 45473 Mülheim an der Ruhr, DE
E-mail: E-mail: E-mail:
DE.Ecobility.Experts@kiwa.com DE.Ecobility.Experts@kiwa.com info@ansorg.com
Website: Website: Website:
https://www.kiwa.com/de/en/themes/ecobility-experts/ecobility-https://www.kiwa.com/de/en/themes/ecobility-experts/ecobility-www.ansorg.com
experts-epd-program/ experts-epd-program/
Kiwa-Ecobility Experts is
established member of the
Punta PXR | ReTHiNK-61567 19 / 19
