ENVIRONMENTAL PRODUCT DECLARATION
as per ISO 14025 and EN 15804+A2
Owner of the Declaration dormakaba International Holding GmbH
Publisher Institut Bauen und Umwelt e.V. (IBU)
Programme holder Institut Bauen und Umwelt e.V. (IBU)
Declaration number EPD-DOR-20210196-CBC1-EN
Issue date 01.10.2021
Valid to 30.09.2026
Reversible Single Cylinder - star plus, neo, primo
dormakaba
www.ibu-epd.com | https://epd-online.com
General Information
dormakaba Reversible Single Cylinder - star plus, neo, primo
Programme holder Owner of the declaration
IBU – Institut Bauen und Umwelt e.V. dormakaba International Holding GmbH
Hegelplatz 1 DORMA Platz 1
10117 Berlin 58256 Ennepetal
Germany Germany
Declaration number Declared product / declared unit
EPD-DOR-20210196-CBC1-EN 1 piece of the product: star plus mechanical key system, consisting of the
following items:
- one (1) star plus single cylinder
- five (5) star plus reversible key
- one (1) security card
- one (1) user manual
- packaging
This declaration is based on the product category rules: Scope:
Building Hardware products, 01.08.2021 This EPD refers to a mechanical key system, including the star plus single
(PCR checked and approved by the SVR) cylinder and five star plus reversible keys. This EPD is also representative
for the products: neo and primo. The underlying life cycle assessment is
based on the entire life cycle of this specific mechanical key system
Issue date manufacured by dormakaba. Data represents the year 2021.
The various technical features are outlined in the product chapter of this
01.10.2021
EPD. The products are manufactured at the dormakaba production facility
in Yokohama (Japan).
The owner of the declaration shall be liable for the underlying information
Valid to
and evidence; the IBU shall not be liable with respect to manufacturer
30.09.2026 information, life cycle assessment data and evidences.
The EPD was created according to the specifications of EN 15804+A2. In
the following, the standard will be simplified as EN 15804.
Verification
The standard EN 15804 serves as the core PCR
Independent verification of the declaration and data according to ISO
14025:2011
internally X externally
Dipl.-Ing. Hans Peters
(Chairman of Institut Bauen und Umwelt e.V.)
Florian Pronold Dr.-Ing. Wolfram Trinius,
(Managing Director Institut Bauen und Umwelt e.V.) (Independent verifier)
1 Environmental Product Declaration - dormakaba - Reversible Single Cylinder - star plus, neo, primo
Product
• Five to eight rows of pins with up to 26 simultaneously-
Product description/Product definition
usable pin positions.
Information about the enterprise
• Pins that make contact with the key are manufactured
dormakaba stands for a broad offering of products, solutions
from wear-resistant hardened steel.
and services for smart and secure access to buildings and
• Key protected by patented characteristic.
rooms from a single source.
• Key of star plus with active protection against copies.
neo is a middle-performance locking system, which is
Product description/ Product definition
registered and factory produced.
star plus, neo and primo are mechanical key systems. They
primo is a basic locking system. Components can be
offer legal protection against commercial imitation. The
assembled at the dealer to be more flexible and faster to deliver
registration of individual locking systems, and master key
to the end customer.
systems with dormakaba ensure that keys cannot be ordered
All systems are available with typical Japanese profile cylinder.
without authorization. Extensions or single parts can be ordered
as required.
Delivery status:
The systems can be used in both the private sector as well as
The declared mechanical key system includes one cylinder and
for large and complex buildings with high security requirements.
five keys, packaging and service instruction with a weight of
star plus, neo and primo can be equipped with RFID
0,476 kg.
transponder for integration in electronic access systems from
dormakaba. Base materials/Ancillary materials
For placing the mechanical key systems on the market in the
For the main product components, the star plus single cylinder
European Union/European Free Trade Association (EU/EFTA,
and five star plus reversible keys the composition of the product
with the exception of Switzerland) the following legal provisions
is the following. Same product composition applies for neo and
apply:
primo:
All systems are classified according to the European locking
cylinder standards EN1303 and DIN18252. While the basic
cylinder configuration already fulfils the attack resistance class
B, the highest protection grade D can be achieved with
integrated carbide steel inserts.
The cylinders and keys contain partial articles which contain
substances listed in the Candidate List of REACH Regulation
dormakaba mechanical cylinders fulfill the material 1907/2006/EC (date:
requirements given within the Directive RoHS 2011/65/EU. 19.01.2021) exceeding 0.1 percentage by mass: yes
• Lead (Pb): 7439-92-1 (CAS-No.) is included in some of
Application
the alloys used. The concentration of lead in each
Reversible mechanical single cylinder can be used in both
individual alloy does not exceed 4.0% (by mass).
residential as well as in the commercial segment and in small
The candidate list can be found on the /ECHA/ website
and simple as well as in large and complex applications, thanks
address: https://echa.europa.eu/de/home
to its versatility. Nearly limitless application options are
possible. Reference service life
The life cycle (security and function) of a lock cylinder is about
Technical Data
10-15 years, depending on the application and frequency of
star plus is a patented high-performance locking systems,
use. The cylinders are tested to 100,000 locking cycles
which fulfills even the most challenging requirements. It has a
minimum (EN1303). This corresponds to approximately 18
virtually unlimited number of locking combinations.
locking cycles per day for 15 years.
The system offers exceptional security thanks to:
LCA: Calculation rules
additional modules: A4 + A5
Declared Unit
The declared unit is 1 piece of the product: star plus Production - Module A1-A3
Declared unit The product stage includes:
— A1, raw material extraction, processing and mechanical
Name Value Unit
treatments, processing of secondary material input (e.g.
Declared unit 1 piece/product
recycling processes), — A2, transport to the manufacturer,
Conversion factor to 1 kg 2.21 - — A3, manufacturing and assembly including provision of all
Mass of declared product including materials, products and energy, as well as waste processing up
0.45247 kg
packaging to the end-of waste state.
System boundary Construction stage - Modules A4-A5
The construction process stage includes:
The type of EPD is according to EN 15804:
— A4, transport to the building site;
"cradle to gate with options, modules C1–C4, and module D".
— A5, installation into the building; including provision of all
The following modules are declared: A1-A3, C1-C4, D and
2 Environmental Product Declaration - dormakaba - Reversible Single Cylinder - star plus, neo, primo
materials, products and energy, as well as waste processing up benefits.
to the end-ofwaste state or disposal of final residues during the
construction process stage. Geographic Representativeness
Land or region, in which the declared product system is
End-of-life stage– Modules C1-C4 and D manufactured, used or handled at the end of the product´s
The end-of-life stage includes: lifespan: Japan
— C1, de-construction, demolition:
— C2, transport to waste processing;
Comparability
— C3, waste processing for reuse, recovery and/or recycling;
Basically, a comparison or an evaluation of EPD data is only
— C4, disposal; including provision and all transport, provision
possible if all the data sets to be compared were created
of all materials, products and related energy and water use.
according to EN 15804 and the building context, respectively
the product-specific characteristics of performance, are taken
Module D (Benefits and loads beyond the system boundary)
into account. Background database: GaBi, SP40.
includes:
— D, recycling potentials, expressed as net impacts and
LCA: Scenarios and additional technical information
Name Value Unit
Characteristic product properties of biogenic carbon
Waste packaging (paper) 0,07682 kg
Information on describing the biogenic Carbon Content at Waste packaging (plastic) 0,00812 kg
factory gate
Name ValueUnit End of life (C1-C4)
Biogenic carbon content in accompanying kg C1: The product dismantling from the building is done manually
packaging 0.033 C without environmental burden.
Name Value Unit
Note: 1 kg of biogenic carbon is equivalent to 44/12 kg of CO .
2
Collected separately waste type 0.36753 kg
Recycling 0.29 kg
The following technical scenario information is required for the Energy recovery 0.07753 kg
declared modules. Disposal 0 kg
Transport to the building site (A4)
The product is disassembled in a recycling process.
Name Value Unit Material recycling is then assumed for the metals. The plastic
Litres of fuel (per piece) 0.0015l/100km components are assumed to be incinerated with energy
recovery.
Transport distance (truck) 1000 km
Capacity utilisation (including empty runs)
55 % Reuse, recovery and/or recycling potentials (D), relevant
average
scenario information
Numbers reflect the average transport distances per cylinder. Collection rate for the cylinder is 100%.
Installation into the building (A5)
3 Environmental Product Declaration - dormakaba - Reversible Single Cylinder - star plus, neo, primo
LCA: Results
DESCRIPTION OF THE SYSTEM BOUNDARY (X = INCLUDED IN LCA; MND = MODULE OR INDICATOR NOT DECLARED; MNR
= MODULE NOT RELEVANT)
Benefits and
Construction loads beyond
Product stage Use stage End of life stage
process stage the system
boundaries
la ire ta m w a Ry lp p u s tro p s n a rT g n iru tc a fu n a M e h t m o rf tro p s n a rTe tis e h t o t e ta g y lb m e s s A e s U e c n a n e tn ia M ria p e R tn e m e c a lp e R tn e m h s ib ru fe R y g re n e la n o ita re p Oe s u re ta w la n o ita re p Oe s u n o itc u rts n o c -e Dn o itilo m e d tro p s n a rT g n is s e c o rp e ts a W la s o p s iD -e s u e R-y re v o c e R-g n ilc y c e Rla itn e to p
A1 A2 A3 A4 A5 B1 B2 B3 B4 B5 B6 B7 C1 C2 C3 C4 D
X X X X X MND MND MNR MNR MNR X MND X X X X X
RESULTS OF THE LCA - ENVIRONMENTAL IMPACT according to EN 15804+A2: 1 piece, Reversible Single Cylinder - star plus,
neo, primo
Parameter Unit A1 A2 A3 A4 A5 B6 C1 C2 C3 C4 D
GWP-total kg CO 2 eq 9.3E-01 4.09E-01 1.97E-01 1.01E-01 1.3E-01 0 0 2E-03 1.97E-01 0 -4.12E-01
GWP-fossil kg CO 2 eq 9.29E-01 4.08E-01 2.84E-01 9.7E-02 2.3E-02 0 0 2E-03 1.97E-01 0 -4.13E-01
GWP-
biogenic kg CO 2 eq -1E-03 1E-03 -8.8E-02 4E-03 1.06E-01 0 0 7.1E-05 4.6E-06 0 1E-03
GWP-luluc kg CO 2 eq 2E-03 8.56E-06 2.13E-04 2.31E-06 2.96E-06 0 0 3.66E-08 1.12E-05 0 -7.07E-04
ODP kg CFC11 eq 1.55E-10 3E-17 8.53E-13 1.02E-17 3E-17 0 0 1.62E-19 9.96E-17 0 -2.42E-15
AP mol H+ eq 9E-03 2E-03 5.46E-04 9.17E-05 3.42E-05 0 0 1.54E-06 3.52E-05 0 -4E-03
EP-
kg P eq 1.23E-06 6.72E-08 2.2E-06 2.07E-08 5.5E-09 0 0 3.29E-10 1.59E-08 0 -3.88E-07
freshwater
EP-marine kg N eq 8.13E-04 7.23E-04 1.81E-04 2.78E-05 1.18E-05 0 0 4.89E-07 7.93E-06 0 -2.79E-04
EP-terrestrial mol N eq 9E-03 8E-03 2E-03 3.12E-04 1.54E-04 0 0 5.44E-06 1.6E-04 0 -3E-03
kg NMVOC
POCP 3E-03 2E-03 5.13E-04 8.11E-05 3.15E-05 0 0 1.38E-06 2.19E-05 0 -9.7E-04
eq
ADPE kg Sb eq 2.68E-04 1.16E-08 3.06E-06 2.91E-09 4.53E-10 0 0 4.61E-11 1.37E-09 0 -1.58E-04
ADPF MJ 1.44E+01 5.54E+00 4E+00 1.37E+00 4.4E-02 0 0 2.2E-02 9.2E-02 0 -5.22E+00
m3 world eq
WDP 3.37E-01 6.25E-04 2.9E-02 1.9E-04 1.6E-02 0 0 3.01E-06 2E-02 0 -1.81E-01
deprived
GWP = Global warming potential; ODP = Depletion potential of the stratospheric ozone layer; AP = Acidification potential of land and water; EP =
Eutrophication potential; POCP = Formation potential of tropospheric ozone photochemical oxidants; ADPE = Abiotic depletion potential for non-fossil
resources; ADPF = Abiotic depletion potential for fossil resources; WDP = Water (user) deprivation potential)
RESULTS OF THE LCA - INDICATORS TO DESCRIBE RESOURCE USE according to EN 15804+A2: 1 piece, Reversible Single
Cylinder - star plus, neo, primo
Parameter Unit A1 A2 A3 A4 A5 B6 C1 C2 C3 C4 D
PERE MJ 1.87E+00 1.3E-02 2.03E+00 4E-03 9.31E-01 0 0 6.87E-05 2.4E-02 0 -9.76E-01
PERM MJ 0 0 9.22E-01 0 -9.22E-01 0 0 0 0 0 0
PERT MJ 1.87E+00 1.3E-02 2.96E+00 4E-03 9E-03 0 0 6.87E-05 2.4E-02 0 -9.76E-01
PENRE MJ 1.13E+01 5.54E+00 3.65E+00 1.38E+00 3.93E-01 0 0 2.2E-02 3.22E+00 0 -5.22E+00
PENRM MJ 3.12E+00 0 3.49E-01 0 -3.49E-01 0 0 0 -3.12E+00 0 0
PENRT MJ 1.44E+01 5.54E+00 4E+00 1.38E+00 4.4E-02 0 0 2.2E-02 9.2E-02 0 -5.22E+00
SM kg 2.38E-01 0 0 0 0 0 0 0 0 0 0
RSF MJ 0 0 0 0 0 0 0 0 0 0 0
NRSF MJ 0 0 0 0 0 0 0 0 0 0 0
FW m3 7E-03 2.6E-05 2E-03 7.77E-06 3.68E-04 0 0 1.23E-07 4.83E-04 0 -4E-03
PERE = Use of renewable primary energy excluding renewable primary energy resources used as raw materials; PERM = Use of renewable primary
energy resources used as raw materials; PERT = Total use of renewable primary energy resources; PENRE = Use of non-renewable primary energy
excluding non-renewable primary energy resources used as raw materials; PENRM = Use of non-renewable primary energy resources used as raw
materials; PENRT = Total use of non-renewable primary energy resources; SM = Use of secondary material; RSF = Use of renewable secondary fuels;
NRSF = Use of non-renewable secondary fuels; FW = Use of net fresh water
RESULTS OF THE LCA – WASTE CATEGORIES AND OUTPUT FLOWS according to EN 15804+A2:
1 piece, Reversible Single Cylinder - star plus, neo, primo
Parameter Unit A1 A2 A3 A4 A5 B6 C1 C2 C3 C4 D
HWD kg 5.65E-06 5.29E-10 3.07E-08 1.33E-10 8.71E-11 0 0 2.12E-12 3.49E-10 0 -1.57E-08
NHWD kg 1.6E-01 5.61E-04 6E-03 1.41E-04 6E-03 0 0 2.23E-06 2.1E-02 0 -9E-02
RWD kg 2.71E-04 4.59E-06 8.9E-05 1.48E-06 2.16E-06 0 0 2.34E-08 3.4E-06 0 -1.66E-04
CRU kg 0 0 0 0 0 0 0 0 0 0 0
MFR kg 0 0 0 0 0 0 0 0 2.9E-01 0 0
MER kg 0 0 0 0 0 0 0 0 0 0 0
4 Environmental Product Declaration - dormakaba - Reversible Single Cylinder - star plus, neo, primo
EEE MJ 0 0 5.1E-02 0 2.03E-01 0 0 0 0 0 0
EET MJ 0 0 9.3E-02 0 3.87E-01 0 0 0 0 0 0
HWD = Hazardous waste disposed; NHWD = Non-hazardous waste disposed; RWD = Radioactive waste disposed; CRU = Components for re-use;
MFR = Materials for recycling; MER = Materials for energy recovery; EEE = Exported electrical energy; EET = Exported thermal energy
RESULTS OF THE LCA – additional impact categories according to EN 15804+A2-optional:
1 piece, Reversible Single Cylinder - star plus, neo, primo
Parameter Unit A1 A2 A3 A4 A5 B6 C1 C2 C3 C4 D
Disease
PM 8.32E-08 5.27E-09 5.02E-09 4.95E-10 2.16E-10 0 0 8.08E-12 4.49E-10 0 -3.79E-08
incidence
IR kBq U235 eq 3.8E-02 6.27E-04 1.4E-02 2.11E-04 3.12E-04 0 0 3.35E-06 3.06E-04 0 -2.8E-02
ETP-fw CTUe 1.07E+01 3.94E+00 1.08E+00 9.74E-01 2E-02 0 0 1.5E-02 3.4E-02 0 -2.95E+00
HTP-c CTUh 1.98E-08 7.38E-11 4.14E-11 1.83E-11 1.17E-12 0 0 2.91E-13 2.97E-12 0 -2.96E-10
HTP-nc CTUh 3.11E-08 3.49E-09 1.73E-09 7.82E-10 6.89E-11 0 0 1.24E-11 3.01E-10 0 -1.47E-08
SQP SQP 4.36E+00 1.1E-02 1.48E+01 4E-03 1.2E-02 0 0 5.6E-05 2.7E-02 0 -2.74E+00
PM = Potential incidence of disease due to PM emissions; IR = Potential Human exposure efficiency relative to U235; ETP-fw = Potential comparative
Toxic Unit for ecosystems; HTP-c = Potential comparative Toxic Unit for humans (cancerogenic); HTP-nc = Potential comparative Toxic Unit for humans
(not cancerogenic); SQP = Potential soil quality index
Disclaimer 1 – for the indicator “Potential Human exposure efficiency relative to U235”. This impact category deals mainly with the
eventual impact of low-dose ionizing radiation on human health of the nuclear fuel cycle. It does not consider effects due to possible
nuclear accidents, occupational exposure or radioactive waste disposal in underground facilities. Potential ionizing radiation from the
soil, radon and from some construction materials is also not measured by this indicator.
Disclaimer 2 – for the indicators “abiotic depletion potential for non-fossil resources”, “abiotic depletion potential for fossil resources”,
“water (user) deprivation potential, deprivation-weighted water consumption”, “potential comparative toxic unit for ecosystems”,
“potential comparative toxic unit for humans – cancerogenic”, “Potential comparative toxic unit for humans - not cancerogenic”,
“potential soil quality index”. The results of this environmental impact indicator shall be used with care as the uncertainties on these
results are high as there is limited experience with the indicator.
References
DIN 18252
DIN 18252: 2018, Profile cylinders for door locks – Terminology, Further References
dimensions, requirements, test methods and marking
IBU
DIN EN 1303 Institut Bauen und Umwelt e.V.: General Instructions for the
DIN EN 1303: 2015, Building Hardware - Cylinders for locks - EPD Programme of Institut Bauen und Umwelt e.V. Version
Requirements and test methods 2.0., Berlin: Institut Bauen und Umwelt e.V., 2021. www.ibu-
epd.com
DIN EN ISO 14025
DIN EN ISO 14025:2011, Environmental labels and GaBi ts software
declarations — Type III environmental declarations - Principles Sphera Solutions GmbH Gabi Software System and Database
and procedures. for Life Cycle Engineering 1992-2020 Version 10.0.0.71
University of Stuttgart, Leinfelden-Echterdingen
EN 15804
EN 15804:2019+A2, Sustainability of construction works — GaBi ts documentation
Environmental Product Declarations — Core rules for the GaBi life cycle inventory data documentation (https://www.gabi-
product category of construction products. software.com/support/gabi/gabidatabase- 2020-lci-
documentation/).
REACH Regulation
REACH Regulation (EC) No 1907/2006 of the European LCA-tool dormakaba
Parliament and of the Council on the Registration, Evaluation, LCA tool, version 1.0.
Authorisation and Restriction of Chemicals. Developed by Sphera Solutions GmbH
RoHS 2011/65/EU PCR Part A
RoHS 2011/65/EU, Directive on the restriction of the use of PCR – Part A: Calculation Rules for the Life Cycle Assessment
certain hazardous substances in electrical and electronic and Requirements on the Project Re-port according to EN
equipment. 15804+A2:2019, Version 1.0, Institut Bauen und Umwelt e.V.,
www.ibu-epd.com.
European Chemicals Agency (ECHA)
https://echa.europa.eu/de/ PCR Part B
PCR – Part B: Requirements on the EPD for Electronic and
physical Access Control Systems , version 1.2, Institut Bauen
und Umwelt e.V., www.ibu-epd.com, 2017.
5 Environmental Product Declaration - dormakaba - Reversible Single Cylinder - star plus, neo, primo
Publisher
Institut Bauen und Umwelt e.V. +49 (0)30 3087748- 0
Hegelplatz 1 info@ibu-epd.com
10117 Berlin www.ibu-epd.com
Germany
Programme holder
Institut Bauen und Umwelt e.V. +49 (0)30 3087748- 0
Hegelplatz 1 info@ibu-epd.com
10117 Berlin www.ibu-epd.com
Germany
Author of the Life Cycle Assessment
Sphera Solutions GmbH +49 711 341817-0
Hauptstraße 111- 113 info@sphera.com
70771 Leinfelden-Echterdingen www.sphera.com
Germany
Owner of the Declaration
dormakaba International Holding GmbH +49 2333 793-0
DORMA Platz 1 info.de@dormakaba.com
58256 Ennepetal www.dormakaba.com
Germany
6 Environmental Product Declaration - dormakaba - Reversible Single Cylinder - star plus, neo, primo
