ENVIRONMENTAL PRODUCT DECLARATION
as per ISO 14025 and EN 15804+A2
Owner of the Declaration Stiferite
Publisher Institut Bauen und Umwelt e.V. (IBU)
Programme holder Institut Bauen und Umwelt e.V. (IBU)
Declaration number EPD-STF-20220332-CBC2-EN
Issue date 16.02.2023
Valid to 15.02.2028
Stiferite FIRE B average thick panel
Stiferite
www.ibu-epd.com | https://epd-online.com
General Information
Stiferite Stiferite FIRE B average thick panel
Programme holder Owner of the declaration
IBU – Institut Bauen und Umwelt e.V. Stiferite
Hegelplatz 1 Viale Navigazione Interna 54
10117 Berlin 35129 Padova
Germany Italy
Declaration number Declared product / declared unit
EPD-STF-20220332-CBC2-EN Stiferite FIRE B average thick panel expanded rigid polyurethane foam,
covered on one side with saturated glass tissue and on the other side with
Stiferite FIRE B facer®, and produced by Stiferite. The EPD applies to 1
m2 of 94.1 mm thick PUR sandwich board, i.e. 0.0941 m3, with an average
density between foam and facing of 38.6 kg/m3.
This declaration is based on the product category rules: Scope:
Insulating materials made of foam plastics, 01.08.2021 Stiferite produces Stiferite FIRE B that is a high performance insulation
(PCR checked and approved by the SVR) board manufactured from closed cell expanded rigid polyurethane foam,
covered on one side with saturated glass tissue and on the other side with
Stiferite Fire B facer®. The data have been provided by the only Stiferite
Issue date factory that is located in Padova (Italy) for the year 2021 and sold
worldwide.
16.02.2023
The owner of the declaration shall be liable for the underlying information
and evidence; the IBU shall not be liable with respect to manufacturer
information, life cycle assessment data and evidences.
Valid to
15.02.2028 The EPD was created according to the specifications of EN 15804+A2. In
the following, the standard will be simplified as EN 15804.
Verification
The standard EN 15804 serves as the core PCR
Independent verification of the declaration and data according to ISO
14025:2011
internally X externally
Dipl.-Ing. Hans Peters
(Chairman of Institut Bauen und Umwelt e.V.)
Dipl.-Ing. Hans Peters Prof. Dr. Birgit Grahl,
(Managing Director Institut Bauen und Umwelt e.V.) (Independent verifier)
1 Environmental Product Declaration - Stiferite - Stiferite FIRE B average thick panel
Product
Association (EU/EFTA) (with the exception of Switzerland)
Product description/Product definition Regulation (EU) No.305/2011 (CPR) applies. The product
Stiferite's thermal insulation panels are mainly used in the needs a Declaration of Performance taking into consideration
building/construction sector and in industrial insulation. EN 13165:2012+A2:2016. Thermal insulation products for
The panels are made of thermo-setting closed cells building- factory made rigid polyurethane foam (PU) products -
polyurethane foam (PU) supplied with various types of flexible Specification and the CE-marking. For the application and use
facers on both sides of the panel. The nature/type of facer is a the respective national provisions apply.
function of the type of panel and its application.
Expanded rigid polyurethane foam is distinguished by its Base materials/Ancillary materials
thermal insulation performance, mechanical resistance, Core material (about 95.8 % of the weight of the declared
workability, lightness, and durability. unit):
The performance of Stiferite's panels is determined based on Closed-cell Polyiso (PIR) rigid foam made from MDI (50-65 %),
the European norm EN13165:2012+A2:2016 Thermal polyols (30-40 %), pentane (4-6 %) and additives (4-6 %).
insulation products for buildings - Factory-made rigid
polyurethane foam (PU) products - Specification. Facing (about 4.2 % of the weight of the declared unit):
This EPD refers to Stiferite's FIRE B mm thick panel, made of consisting of glass fiber (15-25 %), calcium carbonate (55-75
an insulation component in polyurethane foam using blowing %) and graphite (5-15 %).
agent Pentanebased, on one side with saturated glass tissue The PU board for insulation:
and on the other side with Stiferite FIRE B® facer. The
• This product/article/at least one partial article contains
characteristics of the foam and of the facing allow the panel to
substances listed in the candidate list (date: 17.01.2022)
achieve the best reaction to fire class that can be assigned to
exceeding 0.1 percentage by mass: no
organic material.
The panel is produced in standard dimensions of 600 x 1200 • This product/article/at least one partial article doesn't
mm and straight finish borders. contain other carcinogenic, mutagenic, reprotoxic
Upon request and for minimum quantities, the panels may be (CMR) substances in categories 1A or 1B which are not
produced in various dimensions, and the borders may be on the candidate list, exceeding 0.1 percentage by
rabbeted along the sides. The surface of the panel may be mass: no
evened out with sandpaper in order to allow installation on • Biocide products were added to this construction
uneven surfaces. Stiferite FIRE B panel is produced by a product or it has been treated with biocide products (this
certified company with systems:ISO 9001, ISO 45001, ISO then concerns a treated product as defined by the (EU)
14001 in its entire line of products. Ordinance on Biocide Products No.528/2012): no
Application
Additional declaration according to quoted law: The product is
The Stiferite FIRE B panel is recommended in flat roofs: with compliant with all requirements indicated in chapter 2.5.7
cold fixed bituminous or synthetic membrane, Broof t2 and 'Isolanti termici ed acustici' of the n.256 D.L. of the 23th June
Broof t3 certified roofing systems; pitched roof: under roof tiles, 2022 (CAM EDILIZIA):
pantiles or sheet-metal, ventilated; walls: ventilated facades.
• Any blowing agent with Ozone depletion potential >0 is
Technical Data not used in production
In this Life Cycle Assessment, a PU insulation board with the • Any substances of Very High Concern-SVHC in
following properties has been regarded: concentration of more than
0,1 %w are not used in production (REACH n.
Constructional data
1907/2006). Any specific authorizations for use are
Name Value Unit eserved provided for by the same Regulation for the
Gross density 38.6 kg/m3 substances included in Annex XIV and specifications
restrictions set out in Annex XVII of the Regulation.
Declared Average Thermal conductivity λD acc.
0.026 W/mK • Catalysts lead-based are not used in production
to EN 13165
• Flame retardants used in production (belonging to the
Compressive strength at 10% deformation acc.
>150 kPa Organophosphorus class) are not banned by any
to EN 826
national or European regulation
Tensile strength perpendicular to the face acc. >35 kPa • According to the raw materials declarations of suppliers,
to EN 1607 the minimum amount of recycled raw materials based
Water absorption by total immersion acc. to EN Vol.- on the insulation board (PU foam and facers) weight is 3
<2
12087 % % and the minimum amount of recycled raw materials
w
Water absorption by partial immersion acc. to based on the PU insulation foam weight is 4 % in
< 0.1 kg/m² w
EN 1609 compliance with REMADE in Italy type 1 certification
Water vapour diffusion resistance factor μ acc. (note: this information is not explicitly considered in the
56
to EN 12086 LCA and not included in the EPD tables that only refer
B- to recycling content in the foreground system).
Euroclass reaction to fire acc. to EN 11925
s1,d0
Reference service life
This provides a thermal resistance R = 3.6 m² k/W. The durability of insulation panels is normally at least as long as
the lifetime of the building in which it is used. The experimental
Product according to the CPR based on a
data show that the reference life is greater than 50 years.
hEN/:13165:2012+A2:2016 For the placing on the market of the
product in the European Union/European Free Trade
2 Environmental Product Declaration - Stiferite - Stiferite FIRE B average thick panel
LCA: Calculation rules
thermal insulation board. The life cycle is split into the following
Declared Unit individual phases:
The declared unit is 1 m² with a thickness of 94.1 mm, e. g. A1 - Raw material formulation
0.0941 m³. A2 - Raw material transport
Corresponding conversion factors are listed in the table below. A3 - Production of the insulation board and packaging material
Declared unit A4 - Transport to the construction site
C1 - demolition and deconstruction
Name Value Unit
C2 - Transport to end of life
Declared unit 1 m2 C3 - End-of-Life: waste management (thermal recovery)
Gross density 38.6 kg/m3 C4 - End-of-Life: waste management (landfill)
Grammage 3.63 kg/m2 D - Benefits and loads beyond system boundary
Layer thickness 0.0941 m Geographic Representativeness
Declared average thermal conductivity λD 0.026 W/mK Land or region, in which the declared product system is
manufactured, used or handled at the end of the product´s
This provides a thermal resistance R = 3.6 m² /W.
lifespan: Italy
Comparability
System boundary
Basically, a comparison or an evaluation of EPD data is only
Type of the EPD: cradle to gate - with options
possible if all the data sets to be compared were created
This life cycle assessment for the production of the
according to EN 15804 and the building context, respectively
polyurethane insulation board considers the life cycle from the
the product-specific characteristics of performance, are taken
supply of raw materials to the manufacturer´s gate (cradle-to-
into account. The background database used is GaBi 2022
gate with options). It also includes the transport to the
database (v. 2022.1)
construction site and the end-of-life stage of the used PU
LCA: Scenarios and additional technical information
Characteristic product properties of biogenic carbon
End of life (C1-C4)
Name Value Unit
Information on describing the biogenic Carbon Content at
Scenario No 1: Material Incineration 100 %
factory gate
Scenario No 2: Landfill 100 %
Name ValueUnit
kg C1 – Deconstruction and demolition (0.2 MJ/kg as electrical
Biogenic carbon content in product - C consumption assumed)
Biogenic carbon content in accompanying kg
0.003 C2 – Panel is transported from the building site to a treatment
packaging C
plant by truck and an average distance of 100 km is
considered.
C3/C4- Disposal scenarios used are divided into 2 sub-
Transport to the building site (A4) scenarios:
1) Incineration 100 % (C3/1)
Name ValueUnit
2) Landfilling 100 % (C4/2)
Truck with a capacity of 17.3 tons 259 km
Ferry with a capacity of 1200-10000 dwt payload
0 km Reuse, recovery and/or recycling potentials (D), relevant
capacity
scenario information
Ship with a capacity of 27500 dwt payload capacity
0 km D: Benefits and loads beyond system boundary are divided into
tons
2 sub-scenarios:
Plane with a capacity of 22 ton 0 km
Name Value Unit
Type and amount of packaging included in module A3 Scenario No 1: Material Incineration 100 %
Name Value Unit Scenario No 2: Landfill 100 %
Cardboard 0.00691 kg
EPS stock 0.00578 kg
EPS stock - glue 0.00041 kg
Paper labels 0.00014 kg
PE film 0.05808 kg
PP tape 0.00005 kg
PUR stucks 0 kg
SBR labels 0.00001 kg
TOTAL PACKAGING 0.07138 kg
3 Environmental Product Declaration - Stiferite - Stiferite FIRE B average thick panel
LCA: Results
The tables below show the results of the LCA. Basic information on all declared modules provides chapter 4.
There are two scenarios for the end-of-life (C2, C4 and D) analyzed: Scenario 1 considers 100 % incineration, Scenario 2 considers
100 % landfill disposal.
For SM, RSF, NRSF, CRU indicators only the foreground system is considered.
DESCRIPTION OF THE SYSTEM BOUNDARY (X = INCLUDED IN LCA; ND = MODULE OR INDICATOR NOT DECLARED; MNR =
MODULE NOT RELEVANT)
Benefits and
Construction loads beyond
Product stage Use stage End-of-life stage
process stage the system
boundaries
la ire ta m w a Ry lp p u s tro p s n a rT g n iru tc a fu n a M e h t m o rf tro p s n a rTe tis e h t o t e ta g y lb m e s s A e s U e c n a n e tn ia M ria p e R tn e m e c a lp e R tn e m h s ib ru fe R y g re n e la n o ita re p Oe s u re ta w la n o ita re p Oe s u n o itc u rts n o c -e Dn o itilo m e d tro p s n a rT g n is s e c o rp e ts a W la s o p s iD -e s u e R-y re v o c e R-g n ilc y c e Rla itn e to p
A1 A2 A3 A4 A5 B1 B2 B3 B4 B5 B6 B7 C1 C2 C3 C4 D
X X X X MND MND MND MNR MNR MNR MND MND X X X X X
RESULTS OF THE LCA - ENVIRONMENTAL IMPACT according to EN 15804+A2: 1 m2 FIRE B
Parameter Unit A1-A3 A4 C1 C2 C3 C4 D
GWP-total kg CO 2 eq 9.77E+00 8.14E-02 8.3E-02 2.2E-02 7.66E+00 5.43E-02 -3.64E+00
GWP-fossil kg CO 2 eq 9.92E+00 8.06E-02 8.29E-02 2.18E-02 7.66E+00 5.4E-02 -3.64E+00
GWP-biogenic kg CO 2 eq -1.54E-01 2.62E-04 4.89E-05 7.05E-05 5.46E-04 1.68E-04 -3.26E-03
GWP-luluc kg CO 2 eq 5.6E-03 5.44E-04 5.38E-06 1.46E-04 2.12E-05 9.96E-05 -1.97E-04
ODP kg CFC11 eq 1.44E-11 7.92E-15 8.19E-13 2.13E-15 6.49E-13 1.27E-13 -2.68E-11
AP mol H+ eq 1.78E-02 2.86E-04 1.22E-04 7.26E-05 4.55E-03 3.83E-04 -4.5E-03
EP-freshwater kg P eq 3.67E-05 2.88E-07 3.72E-08 7.76E-08 1.99E-07 9.15E-08 -1.27E-06
EP-marine kg N eq 4.99E-03 1.32E-04 3.33E-05 3.32E-05 2.2E-03 9.79E-05 -1.31E-03
EP-terrestrial mol N eq 5.03E-02 1.48E-03 3.56E-04 3.72E-04 2.53E-02 1.08E-03 -1.41E-02
kg NMVOC
POCP 1.95E-02 2.58E-04 9.4E-05 6.51E-05 5.65E-03 2.97E-04 -3.73E-03
eq
ADPE kg Sb eq 5.81E-06 8.13E-09 9.86E-09 2.19E-09 1.72E-08 5.54E-09 -3.66E-07
ADPF MJ 2.49E+02 1.06E+00 1.76E+00 2.85E-01 2.26E+00 7.07E-01 -7.23E+01
m3 world eq
WDP 2.15E+00 9.03E-04 6.19E-03 2.43E-04 7.72E-01 5.92E-03 -2.05E-01
deprived
GWP = Global warming potential; ODP = Depletion potential of the stratospheric ozone layer; AP = Acidification potential of land and water; EP =
Eutrophication potential; POCP = Formation potential of tropospheric ozone photochemical oxidants; ADPE = Abiotic depletion potential for non-fossil
resources; ADPF = Abiotic depletion potential for fossil resources; WDP = Water (user) deprivation potential)
RESULTS OF THE LCA - INDICATORS TO DESCRIBE RESOURCE USE according to EN 15804+A2: 1 m2 FIRE B
Parameter Unit A1-A3 A4 C1 C2 C3 C4 D
PERE MJ 1.43E+01 7.34E-02 2.54E-01 1.98E-02 3.82E-01 1.06E-01 -8.35E+00
PERM MJ 1.2E-01 ND ND ND ND ND ND
PERT MJ 1.44E+01 7.34E-02 2.54E-01 1.98E-02 3.82E-01 1.06E-01 -8.35E+00
PENRE MJ 1.53E+02 1.06E+00 1.76E+00 2.86E-01 9.58E+01 9.42E+01 -7.23E+01
PENRM MJ 9.66E+01 ND ND ND -9.35E+01 -9.35E+01 ND
PENRT MJ 2.49E+02 1.06E+00 1.76E+00 2.86E-01 2.27E+00 7.08E-01 -7.23E+01
SM kg 4.24E-01 ND ND ND ND ND ND
RSF MJ ND ND ND ND ND ND ND
NRSF MJ ND ND ND ND ND ND ND
FW m3 6.91E-02 8.48E-05 3.85E-04 2.28E-05 1.82E-02 1.8E-04 -1.27E-02
PERE = Use of renewable primary energy excluding renewable primary energy resources used as raw materials; PERM = Use of renewable primary
energy resources used as raw materials; PERT = Total use of renewable primary energy resources; PENRE = Use of non-renewable primary energy
excluding non-renewable primary energy resources used as raw materials; PENRM = Use of non-renewable primary energy resources used as raw
materials; PENRT = Total use of non-renewable primary energy resources; SM = Use of secondary material; RSF = Use of renewable secondary fuels;
NRSF = Use of non-renewable secondary fuels; FW = Use of net fresh water
RESULTS OF THE LCA – WASTE CATEGORIES AND OUTPUT FLOWS according to EN 15804+A2:
1 m2 FIRE B
Parameter Unit A1-A3 A4 C1 C2 C3 C4 D
HWD kg 6.31E-08 5.63E-12 1.26E-10 1.51E-12 3.01E-10 3.64E-11 -6.82E-09
NHWD kg 2.53E-01 1.73E-04 3.74E-04 4.66E-05 1.07E-01 3.62E+00 -1.61E-02
RWD kg 2.87E-03 1.97E-06 2.92E-04 5.31E-07 1.06E-04 7.9E-06 -9.55E-03
CRU kg ND ND ND ND ND ND ND
MFR kg ND ND ND ND ND ND ND
MER kg ND ND ND ND ND ND ND
4 Environmental Product Declaration - Stiferite - Stiferite FIRE B average thick panel
EEE MJ ND ND ND ND 2.36E+01 ND ND
EET MJ ND ND ND ND 1.32E+01 ND ND
HWD = Hazardous waste disposed; NHWD = Non-hazardous waste disposed; RWD = Radioactive waste disposed; CRU = Components for re-use;
MFR = Materials for recycling; MER = Materials for energy recovery; EEE = Exported electrical energy; EET = Exported thermal energy
RESULTS OF THE LCA – additional impact categories according to EN 15804+A2-optional:
1 m2 FIRE B
Parameter Unit A1-A3 A4 C1 C2 C3 C4 D
Disease
PM 1.38E-07 1.66E-09 1.09E-09 4.15E-10 1.33E-08 4.71E-09 -3.99E-08
incidence
IR kBq U235 eq 3.34E-01 2.98E-04 4.28E-02 8.02E-05 1.66E-02 8.8E-04 -1.4E+00
ETP-fw CTUe 1.05E+02 7.51E-01 5.38E-01 2.02E-01 7.77E-01 1.29E+01 -1.77E+01
HTP-c CTUh 6.85E-09 1.55E-11 9.91E-12 4.16E-12 5.45E-11 6.05E-11 -4.38E-10
HTP-nc CTUh 6.2E-07 9.64E-10 5.04E-10 2.55E-10 2.09E-09 6.7E-09 -2.12E-08
SQP SQP 3.14E+01 4.48E-01 1.61E-01 1.21E-01 4.52E-01 1.47E-01 -5.31E+00
PM = Potential incidence of disease due to PM emissions; IR = Potential Human exposure efficiency relative to U235; ETP-fw = Potential comparative
Toxic Unit for ecosystems; HTP-c = Potential comparative Toxic Unit for humans (cancerogenic); HTP-nc = Potential comparative Toxic Unit for humans
(not cancerogenic); SQP = Potential soil quality index
Disclaimer 1 – for the indicator “Potential Human exposure efficiency relative to U235”. This impact category deals mainly with the
eventual impact of low-dose ionizing radiation on human health of the nuclear fuel cycle. It does not consider effects due to possible
nuclear accidents, occupational exposure or radioactive waste disposal in underground facilities. Potential ionizing radiation from the
soil, radon and from some construction materials is also not measured by this indicator.
Disclaimer 2 – for the indicators “abiotic depletion potential for non-fossil resources”, “abiotic depletion potential for fossil resources”,
“water (user) deprivation potential, deprivation-weighted water consumption”, “potential comparative toxic unit for ecosystems”,
“potential comparative toxic unit for humans – cancerogenic”, “Potential comparative toxic unit for humans - not cancerogenic”,
“potential soil quality index”. The results of this environmental impact indicator shall be used with care as the uncertainties on these
results are high as there is limited experience with the indicator.
References
Standards products -Specification
CPR EN 15804
Regulation (EU) No.305/2011 laying down harmonised EN 15804:2012+A2:2019+AC:2021 Sustainability of
conditions for the marketing of construction products and construction works — Environmental Product Declarations —
repealing Council Directive 89/106/EEC Core rules for the product category of construction products.
EN 826 ISO 9001
EN 826:2013 Determination of Compression Behavior of ISO 9001:2015 Quality management
Thermal Insulation Products
ISO 14001
EN 1607 ISO 14001: 2015 Environmental management systems
EN 1607:2013 Thermal insulating products for building
applications. Determination of tensile strength perpendicular to ISO 14025
faces EN ISO 14025:2011 Environmental labels and declarations —
Type III environmental declarations - Principles and procedures.
EN 1609
EN 1609: Thermal insulating products for building ISO 45001
applications.Determination of short term water absorption by ISO 45001: 2018 Occupational health and safety management
partial immersion. systems
EN 11925 GaBi 2022
EN 11925:2010 Reaction to fire tests. Ignitability of products GaBi 10 and DB 2022.1: Documentation of GaBi 10: Software-
subjected to direct impingement of flame. Single-flame source System and Database for Life Cycle Engineering. Copyright,
test. TM. Stuttgart, Leinfelden-Echterdingen, 1992-2022
http://www.gabi-software.com
EN 12086
EN 12086:2013 Thermal insulating products for building IBU 2021
applications. Determination of water vapour transmission Institut Bauen und Umwelt e.V.: General Instructions for the
properties. EPD programme of Institut Bauen und Umwelt e.V.,Version 2.0,
Berlin: Institut Bauen und Umwelt e.V., 2021
EN 12087 www.ibu-epd.com
EN 12087:2013 Thermal insulating products for building
applications. Determination of long term water absorption by IBU PCR Part A
immersion. Product Category Rules for Building-Related Products and
Services. Part A: Calculation Rules for the Life Cycle
EN 13165 Assessment and Requirements on the Project Report according
EN 13165:2012+A2:2016 Thermal insulation products for to EN 15804+A2:2019; V1.2, 11/2021
buildings - Factory made rigid polyurethane foam (PU)
5 Environmental Product Declaration - Stiferite - Stiferite FIRE B average thick panel
IBU PCR Part B REACH
PCR Guidance-Texts for Building-Related Productsand REACH Registration, Evaluation, Authorization and Restriction
Services; Part B: Requirements on the EPD for Insulating of Chemical, 2007
materials made of foam plastics; Institute Construction and
Environment e.V. (IBU). Version 01.2019 REMADE IN ITALY
https://epd-online.com Certificate No.1245/001 for Stiferite Rev. n. 0 18 November
2021
PANGPP 2022
Piano d' Azione Nazionale sul Green Public Procurement Ordinance on Biocide Products
(PANGPP) – Decreto Ministeriale n. 256 del 23-06-2022 Regulation (eu) n. 528/2012 of the European Parliament and of
Gazzetta Ufficiale della Repubblica Italiana, Serie Generale the Council of 22 May 2012 concerning the making available on
n.183 del 06-08-2022 the market and use of biocidal products Text with EEA
https://www.mite.gov.it/notizie/novita-sui-criteri-minini- relevance
ambientali-cam
STIFERITE LCA tool background report v 2.3 (03-06-2022)
6 Environmental Product Declaration - Stiferite - Stiferite FIRE B average thick panel
Publisher
Institut Bauen und Umwelt e.V. +49 (0)30 3087748- 0
Hegelplatz 1 info@ibu-epd.com
10117 Berlin www.ibu-epd.com
Germany
Programme holder
Institut Bauen und Umwelt e.V. +49 (0)30 3087748- 0
Hegelplatz 1 info@ibu-epd.com
10117 Berlin www.ibu-epd.com
Germany
Author of the Life Cycle Assessment
Sphera Solutions GmbH +49 711 341817-0
Hauptstraße 111- 113 info@sphera.com
70771 Leinfelden-Echterdingen www.sphera.com
Germany
Owner of the Declaration
Stiferite +39 049 8997911
Viale Navigazione Interna 54 info@stiferite.com
35129 Padova www.stiferite.com
Italy
7 Environmental Product Declaration - Stiferite - Stiferite FIRE B average thick panel
