ENVIRONMENTAL PRODUCT DECLARATION
as per /ISO 14025/ and /EN 15804/
Owner of the Declaration Etex Building Performance International
Programme holder Institut Bauen und Umwelt e.V. (IBU)
Publisher Institut Bauen und Umwelt e.V. (IBU)
Declaration number EPD-ETX-20190100-IBA1-EN
Issue date 08.01.2020
Valid to 07.01.2025
HYDROPANEL
Fibre cement drywall panels
Etex Building Performance International
www.ibu-epd.com / https://epd-online.com
Umwelt Produktdeklaration Name des Herstellers – Name des Produkts
1. General Information
Etex Building Performance International Hydropanel Drywall Panel
Programme holder Owner of the declaration
IBU - Institut Bauen und Umwelt e.V. Etex Building Performance International
Panoramastr. 1 500 rue Marcel Demonque
10178 Berlin 84915 Avignon Cedex 9
Germany FRANCE
Declaration number Declared product / declared unit
EPD-ETX-20190100-IBA1-EN 1m² Hydropanel
This declaration is based on the product Scope:
category rules: The Environmental Product Declaration includes the
Fibre cement / Fibre concrete, 07.2014 environmental parameters for the Hydropanel drywall
(PCR checked and approved by the SVR) panels produced by Etex Building performance
International. The result of the life cycle assessment
provided in this EPD is based on a thickness of 9mm.
Issue date
This document refers to the structural panels
08.01.2020
manufactured in the Kapelle-op-den-Bos plant
(Belgium). The production data used refers to the
Valid to
production year 2016. Based on plausible, transparent
07.01.2025 and comprehensible basic data, the Life Cycle
Assessment fully represents the Etex products in
question.
In an annex to this EPD the LCA results for additional
thicknesses (6 mm and 12 mm) are declared.
The owner of the declaration shall be liable for the
underlying information and evidence; the IBU shall not
be liable with respect to manufacturer information, life
cycle assessment data and evidences.
Verification
The standard /EN 15804/ serves as the core PCR
Independent verification of the declaration and data
according to /ISO 14025:2010/
Dipl. Ing. Hans Peters internally x externally
(President of Institut Bauen und Umwelt e.V.)
Dr. Alexander Röder Dipl. Natw. ETH Sascha Iqbal
(Head of Board IBU) (Independent verifier appointed by SVR)
2. Product
2.1 Product description / Product definition
This Environmental Product Declaration refers to large- External monitoring of the products with general
format structural panels comprising cellulose- technical approval by the Material Testing Institute of
reinforced fibre-cement panels. The products under the state of Brandenburg/Berlin and the German
review involve smooth panels made from steam- Federal Institute for Materials Research and Testing
hardened fibre cement. (/BAM/).
For the placing on the market of the product in the For the application and the use, the respective national
European Union / European Free Trade Association provisions apply.
(EFTA) (with the exception of Switzerland) the
/Construction Products Regulation/ applies. The 2.2 Application
product needs a declaration of performance taking into Hydropanel is a building board for interior areas
consideration /EN 12467/: Fibre-cement flat sheets - exposed to high levels of humidity. It serves as a
Product specification and test methods. backer board for tiles and moisture-resistant top coat
systems.
CE Declaration of Conformity in accordance with the
specifications outlined in Annex ZA to /EN 12467/. 2.3 Technical Data
General technical approval no. /Z-31.4-160/ of the Sound insulation:
"Deutsches Institut für Bautechnik" (DIBt).
2 Environmental Product Declaration ETEX – Hydropanel Fibre-Cement Drywall Panels
A sound insulation value of Rw = 54 dB is achieved in This product contains other carcinogenic, mutagenic
a reinforced steel partition wall system with metal and toxic for reproduction (CMR) substances in
profiles 50 mm in depth, cladding on both sides with 2 categories 1A or 1B which are not on the candidate
x 12 mm Hydropanel and the reinforced steel partition list, exceeding 0.1 % by mass: no
wall lined with 40 mm mineral wool infill.
Standard-related tests for CE marking via type testing Biocide products were added to this construction
in accordance with /EN 12467/. product or it has been treated with biocide products
(this then concerns a treated product as defined by the
Constructional data (EU) /Ordinance on Biocide Products/):
Name Value Unit no
Gross density dry, mean, +/- 10% 1180 kg/m3
Compressive strength 38 N/mm2 2.6 Manufacture
Modulus of elasticity perpendicular >7.5 N/mm2 Large-format panels made of fibre cement are
Modulus of elasticity parallel >8.5 N/mm² manufactured mainly in accordance with an automated
Flexural strength perpendicular >10.4 N/mm2 winding process. The raw materials are treated with
Flexural strength parallel >16.9 N/mm² water to form a homogeneous mixture. Rotating screen
Tensile strength 6.3 N/mm2 cylinders are immersed in this fibre cement pulp which
drains the mixture outwards.
Water vapour diffusion resistance 84 (wet) -
- The screen surface is coated with a thin fibre cement
factor 143 (dry)
film which is conveyed onto an infinite transport belt
Moisture content at 23 °C, 80%
6 M.-% from where it reaches a format roller to which an
humidity
increasingly thick layer of fibre cement is applied. Once
Coefficient of thermal expansion <6.5 10-6K-1
the requisite material thickness has been achieved, the
Swelling (air-dry to water-
7 mm/m still moist and malleable fibre cement layer (fibre
saturated)
cement fleece) is unravelled and detached from the
similar to
format roller.
Chemical resistance concrete -
The fibre cement fleece is cut to length and any
C35/C45
leftovers are returned to the production process with
similar to
the result that no waste is incurred. The panels are
Ageing resistance concrete -
then set aside for binding before stacking on pallets
C35/C45
and steam-hardened in an autoclave for approx. 2
Permanent temperature
up to 100 °C hours. The setting time lasts approx. 3 days.
resistance
Thermal conductivity 0.19 W/(mK)
Quality Management
The production facilities are TÜV-certified in
accordance with /ISO 9001/.
Performance data of the product in accordance with
the declaration of performance with respect to its 2.7 Environment and health during
essential characteristics according to /EN 12467/. manufacturing
During the entire manufacturing process, there are no
2.4 Delivery status other health protection measures extending beyond
The Hydropanel is delivered with a maximum size of the legally specified industrial protection measures for
3.100 mm x 1.500 mm in three strenghts of 6 mm, 9 commercial enterprises.
mm and 12 mm and with a smooth surface.
 Air: Any dust incurred is collected in filter
systems and partially re-used. Emissions are
2.5 Base materials / Ancillary materials
significantly lower than the limit values
Base materials in % mass (dry mass)
specified by the TA Air.
 25-45% Portland cement to /EN 197-1/, (CEM  Water/Soil: Water incurred during
I 32.5 R and 42.5 R) (binding agent) manufacturing and plant cleaning is treated
 25-45% Quartz sand, mineral aggregates mechanically in waste water treatment
 1-15% Wollastonite systems on the plant site and re-used in the
 1-10% Cellulose fibres production process.
 1-10% Mica  Noise: The noise emissions into the
 1-10% Aluminium hydroxide environment by production equipment fall
short of the permissible limit values.
and water for mixing the cement: 0.24 m³/t fibre
cement. The production facilities are certified in accordance
Cellulose-reinforced fibre cement products were with /ISO 14001/ and /OHSAS 18001/.
introduced in 1980s as a safe replacement for the
widely used asbestos cement products manufactured 2.8 Product processing/Installation
before that time. Special low-dust equipment such as slow-running,
Information that product does not contain substances carbide-tipped splitting saws or cutting burs are
listed in the Candidate List of substances of very high available for processing. Drill holes can be made using
concern (/REACH Regulation/) exceeding 0.1%: standard high-speed steel twist (HSS) drills. Additional
This product contains substances listed in the products required for installing the products under
candidate list (date: 15.01.2019) exceeding 0.1 % by review include: wood or metal substructures including
mass: no the requisite anchoring and joining components as well
as securing parts (screws, nails, staples). When
3 Environmental Product Declaration ETEX – Hydropanel Fibre-Cement Drywall Panels
selecting any requisite constructive products, please Combustion gases: the results in line with testing to
ensure that they do not have a negative influence on /DIN 53436/ indicate that the gaseous emissions
the designated function of the construction products incurred when burning the panels in question are free
referred to. of sulphur and chlorine compounds. The concentration
The set of rules laid out by the employers' liability of released hydrogen cyanide (HCN) is within a normal
insurance associations shall apply. framework.
When processing the products under review,
conventional industrial protection measures must be Changing the system condition (burning dripping/falling
observed in accordance with information supplied by material): When surrounding construction materials are
the manufacturer. Please note that dust generated burned, the cellulose fibres bound in the cement
during processing can have an alkaline reaction (pH gradually lose their strength: This does not represent
value: >10). any explosive potential with the result that fibre cement
According to the present state of knowledge, hazards does not pose a risk in the event of a fire. Burning
for water, air and soil can not arise when fibre cement dripping/falling hydrophobic treatment or fibre cement
is processed as designated. do not occur.
2.9 Packaging
Cardboard boxes, wooden pallets and steel bands are Water
used as packaging materials. The wooden pallets can No ingredients are washed out which could be
be returned by the customer and reused several times. hazardous to water (see also “Eluate analysis” in
Evidence). The pH value is alkaline (pH ≥ 10).
2.10 Condition of use Mechanical destruction
Hydration of the cement and water mixture forms Not of relevance
hardened cement paste (calcium silicate hydrate) with
embedded fibres and fillers as well as micro air pores. 2.14 Re-use phase
The fibre-cement products comprise approx. 6% water De-construction: depending on the mounting system,
(equilibrium moisture) and a proportion by volume of the structural panels can be removed non-destructively
approx. 30% air (contained in the micro-pores). by unscrewing or opening the studs.
After the binding agent has set and when used as
designated, fibre cement products can be used for Re-use / further use: if undamaged, de-constructed
practically any applications. No maintenance or repair panels can be re-used as backer board or as
is required over the service life of the boards. foundation protection.
2.11 Environment and health during use Re-use / Further use: when separated by type, fibre-
Environmental protection: According to the present cement products referred to can be re-ground and re-
state of knowledge, hazards for water, air and soil used as additives in the manufacture of fibre cement
cannot arise when the products under review are (material recycling). When sorted by type, the fibre-
processed as designated (see chapter 7). cement products in question are also suitable for
further use as a filler and loose material in civil
Health protection: When the construction products engineering, especially in road construction or for
are used as designated, no health hazards are known noise barriers (material recycling).
in connection with the base materials used and the
performance thereof in the condition of use (see 2.15 Disposal
chapter 7). Within the production process, most of the generated
waste is immediately re-used within the process.
2.12 Reference service life When after end-of-life re-using or recycling the boards
When used in partition walls, the service life of as described in the previous paragraph is not practical,
Hydropanel is comparable with the reference service the boards can be disposed to landfill class II.
life (RSL) of plasterboard. The waste code in accordance with the /European
The service life according to the "Bundesinstitut für Waste Index/ is 170904.
Bau-, Stadt- und Raumforschung" (/BBSR/) table is
indicated to be > 50 years. 2.16 Further information
Further information is available on the following
website: www.siniat.de.
2.13 Extraordinary effects
Fire
Building materials class A2 as per /DIN 4102-1/, i.e.
limited combustibility.
Building materials classification to /EN 13501-1/ A2,s1-
d0, i.e. limited combustibility in accordance with Part A
of the Building Rules List.
Development of smoke/smoke density: smoke
development caused by burning the products in
question (coating) is very low.
4 Environmental Product Declaration ETEX – Hydropanel Fibre-Cement Drywall Panels
3. LCA: Calculation rules
3.1 Declared Unit and electric power consumption as well as waste
This declaration refers to the production of 1m2 management processes using best available life cycle
Hydropanel (9mm, grammage 11.7 kg/m²) inventory (LCI) datasets. This includes input flows with
manufactured in Kapelle-op-den-Bos, Belgium. a contribution of less than 1% of mass or energy.
Production of capital equipment, facilities and
Declared unit infrastructure required for manufacture are outside the
Name Value Unit scope of this assessment.
Declared unit 1 m²
Gross density * 1290 kg/m3 3.5 Background data
* within range of 1180 kg/m³ +- 10% The /GaBi ts software/ was used to model the product
life cycle. The basic data in the GaBi database is
applied for energy, transportation, auxiliary products
3.2 System boundary and preliminary products. The software was revised in
Type of EPD: Cradle-to-gate with options. 2018.
The following life cycle stages and modules are Hydropanel is produced in Belgium. Belgian datasets
included: were used for the grid mixes. For other processes for
which no Belgian datasets were available, European
Production stage (A1-A3): average datasets were used (EU-28).
 transportation and manufacturing of pre-
3.6 Data quality
products to the manufacturing site
The overall data quality and quality of the data
 energy consumption and use of auxiliary
collection can be described as good. All relevant flows
materials during production
were considered. Methodological choices are
 disposal of production wastes consistent throughout the model.
 production of packaging
3.7 Period under review
Etex provided production data based on an annual
Construction stage (A4-A5):
average of the year 2016.
 transportation of product to the construction
site 3.8 Allocation
 energy consumption during the installation of Production data refer to the declared product allocated
products from the overall production volume (m2 virtually
normalised to 5 mm thickness) in Kapelle-op-den-Bos,
 production of fixing- and finishing material
Belgium.
 disposal of installation wastes including
Specific information on allocation within the
emissions of biogenic CO from cellulose
2 background data is given in the /GaBi documentation/
 disposal/incineration of packaging materials (http://www.gabi-
(potential benefits from energy substitution software.com/international/support/gabi/gabi-database-
within the incineration process are declared in 2018-lci-documentation/).
module D) including emissions of biogenic
3.9 Comparability
CO from renewable packaging materials
2 Basically, a comparison or an evaluation of EPD data
is only possible if all the data sets to be compared
Use stage (B1-B7): were created according to /EN 15804/ and the building
 efforts for the use of the product, context, respectively the product-specific
maintenance and operational efforts characteristics of performance, are taken into account.
GaBi ts serves as background database for the
End-of-life stage (C1-C4): calculation of the life cycle assessment /GaBi ts
 energy consumption for de-construction and software/
demolition
 transportation to disposal
 waste processing and landfilling of product
.
3.3 Estimates and assumptions
No estimations or assumptions were made for the
production stage. Information on assumptions for the
scenarios in the life cycle of the product are described
in chapter 4.
3.4 Cut-off criteria
All available data from production processes were
considered, i.e., all pre-products used, thermal energy
4. LCA: Scenarios and additional technical information
5 Environmental Product Declaration ETEX – Hydropanel Fibre-Cement Drywall Panels
Transport to the building site (A4)
Name Value Unit
Transport distance 600 km
Capacity utilisation (including
61 %
empty runs)
Installation into the building (A5)
Name Value Unit
Auxiliary Steel screws 0.128 kg
Water consumption 0.000161 m3
Other resources : Powder mix
0.35 kg
finisher
Electricity consumption 0.02 kWh
Material loss 0.35 kg
Dust in the air * 0 kg
VOC in the air 0 kg
* See chapter 2.8 for details regarding prevention of
dust emissions.
Use or application of the installed product (B1) see
section 2.11 "Use"
No efforts and releases of substances occur during the
normal (i.e. anticipated) use phase.
Maintenance (B2)
No efforts occur during maintenance.
Name Value Unit
Water consumption 0 m3
Auxiliary 0 kg
Other resources 0 kg
Electricity consumption 0 kWh
Other energy carriers 0 MJ
Waste materials resulting from
0 kg
maintenance
Operational energy use (B6) and Operational water
use (B7)
No efforts occur in modules B6 and B7. m2
Name Value Unit
Water consumption 0 m3
Electricity consumption 0 kWh
Other energy carriers 0 MJ
End of life (C1-C4)
Name Value Unit
Collected as mixed construction
12.2 kg
waste (incl. finisher and screws)
Recycling 0.1 kg
Landfilling 12.1 kg
6 Environmental Product Declaration ETEX – Hydropanel Fibre-Cement Drywall Panels
5. LCA: Results
DESCRIPTION OF THE SYSTEM BOUNDARY (X = INCLUDED IN LCA; MND = MODULE NOT DECLARED)
BENEFITS AND
CONSTRUCTI LOADS
PRODUCT STAGE ON PROCESS USE STAGE END OF LIFE STAGE BEYOND THE
STAGE SYSTEM
BOUNDARIES
7 Environmental Product Declaration ETEX – Hydropanel Fibre-Cement Drywall Panels
lairetam
waR
ylppus tropsnarT
gnirutcafunaM
eht
morf
tropsnarT
etis
eht
ot
etag
ylbmessA esU
ecnanetniaM
riapeR
tnemecalpeR tnemhsibrufeR
ygrene
lanoitarepO esu
retaw
lanoitarepO esu
noitcurtsnoc-eD
noitilomed tropsnarT
gnissecorp
etsaW
lasopsiD -esueR -yrevoceR -gnilcyceR laitnetop
A1 A2 A3 A4 A5 B1 B2 B3 B4 B5 B6 B7 C1 C2 C3 C4 D
X X X X X X X MNR MNR MNR X X X X X X X
RESULTS OF THE LCA - ENVIRONMENTAL IMPACT: 1 m² Hydropanel (9 mm)
Param
Unit A1-A3 A4 A5 B1 B2 B6 B7 C1 C2 C3 C4 D
eter
GWP [kg CO2-Eq.] 5.78E+0 4.44E-1 9.73E-1 0.00E+0 0.00E+0 0.00E+0 0.00E+0 8.61E-3 3.83E-2 0.00E+0 1.56E+0 -1.96E-1
ODP [kg CFC11-Eq.] 4.73E-12 1.21E-14 7.15E-11 0.00E+0 0.00E+0 0.00E+0 0.00E+0 3.83E-14 1.04E-15 0.00E+0 6.25E-14 3.85E-14
AP [kg SO2-Eq.] 1.51E-2 1.03E-3 2.32E-3 0.00E+0 0.00E+0 0.00E+0 0.00E+0 2.44E-5 8.87E-5 0.00E+0 1.39E-3 -4.72E-4
EP [kg (PO4)3--Eq.] 2.29E-3 2.62E-4 3.48E-4 0.00E+0 0.00E+0 0.00E+0 0.00E+0 2.29E-6 2.26E-5 0.00E+0 2.18E-3 -4.04E-5
POCP [kg ethene-Eq.] 1.26E-3 -3.49E-4 2.64E-4 0.00E+0 0.00E+0 0.00E+0 0.00E+0 1.53E-6 -3.01E-5 0.00E+0 4.25E-4 -6.06E-5
ADPE [kg Sb-Eq.] 6.29E-6 3.63E-8 2.46E-5 0.00E+0 0.00E+0 0.00E+0 0.00E+0 4.57E-9 3.13E-9 0.00E+0 8.54E-8 2.02E-8
ADPF [MJ] 5.92E+1 6.01E+0 8.40E+0 0.00E+0 0.00E+0 0.00E+0 0.00E+0 9.16E-2 5.19E-1 0.00E+0 3.48E+0 -1.55E+0
GWP = Global warming potential; ODP = Depletion potential of the stratospheric ozone layer; AP = Acidification potential of land and water; EP =
Caption Eutrophication potential; POCP = Formation potential of tropospheric ozone photochemical oxidants; ADPE = Abiotic depletion potential for non-
fossil resources; ADPF = Abiotic depletion potential for fossil resources
RESULTS OF THE LCA - RESOURCE USE: 1 m² Hydropanel (9 mm)
Parameter Unit A1-A3 A4 A5 B1 B2 B6 B7 C1 C2 C3 C4 D
PERE [MJ] 1.80E+1 3.33E-1 2.52E+0 0.00E+0 0.00E+0 0.00E+0 0.00E+0 5.91E-2 2.87E-2 0.00E+0 3.84E-1 1.42E-1
PERM [MJ] 1.00E+1 0.00E+0 0.00E+0 0.00E+0 0.00E+0 0.00E+0 0.00E+0 0.00E+0 0.00E+0 0.00E+0 0.00E+0 0.00E+0
PERT [MJ] 2.80E+1 3.33E-1 2.52E+0 0.00E+0 0.00E+0 0.00E+0 0.00E+0 5.91E-2 2.87E-2 0.00E+0 3.84E-1 1.42E-1
PENRE [MJ] 6.87E+1 6.04E+0 9.52E+0 0.00E+0 0.00E+0 0.00E+0 0.00E+0 1.57E-1 5.21E-1 0.00E+0 3.61E+0 -1.46E+0
PENRM [MJ] 0.00E+0 0.00E+0 0.00E+0 0.00E+0 0.00E+0 0.00E+0 0.00E+0 0.00E+0 0.00E+0 0.00E+0 0.00E+0 0.00E+0
PENRT [MJ] 6.87E+1 6.04E+0 9.52E+0 0.00E+0 0.00E+0 0.00E+0 0.00E+0 1.57E-1 5.21E-1 0.00E+0 3.61E+0 -1.46E+0
SM [kg] 3.07E-1 0.00E+0 9.19E-3 0.00E+0 0.00E+0 0.00E+0 0.00E+0 0.00E+0 0.00E+0 0.00E+0 0.00E+0 0.00E+0
RSF [MJ] 0.00E+0 0.00E+0 0.00E+0 0.00E+0 0.00E+0 0.00E+0 0.00E+0 0.00E+0 0.00E+0 0.00E+0 0.00E+0 0.00E+0
NRSF [MJ] 0.00E+0 0.00E+0 0.00E+0 0.00E+0 0.00E+0 0.00E+0 0.00E+0 0.00E+0 0.00E+0 0.00E+0 0.00E+0 0.00E+0
FW [m³] 2.57E-2 6.13E-4 5.20E-3 0.00E+0 0.00E+0 0.00E+0 0.00E+0 8.05E-5 5.29E-5 0.00E+0 6.12E-4 6.89E-5
PERE = Use of renewable primary energy excluding renewable primary energy resources used as raw materials; PERM = Use of
renewable primary energy resources used as raw materials; PERT = Total use of renewable primary energy resources; PENRE = Use of
non-renewable primary energy excluding non-renewable primary energy resources used as raw materials; PENRM = Use of non-
Caption
renewable primary energy resources used as raw materials; PENRT = Total use of non-renewable primary energy resources; SM = Use
of secondary material; RSF = Use of renewable secondary fuels; NRSF = Use of non-renewable secondary fuels; FW = Use of net fresh
water
RESULTS OF THE LCA – OUTPUT FLOWS AND WASTE CATEGORIES:
1 m² Hydropanel (9 mm)
Parameter Unit A1-A3 A4 A5 B1 B2 B6 B7 C1 C2 C3 C4 D
HWD [kg] 2.87E-7 3.49E-7 1.72E-4 0.00E+0 0.00E+0 0.00E+0 0.00E+0 7.37E-11 3.01E-8 0.00E+0 4.56E-8 -1.00E-9
NHWD [kg] 4.66E-1 5.06E-4 3.75E-1 0.00E+0 0.00E+0 0.00E+0 0.00E+0 1.11E-4 4.36E-5 0.00E+0 1.18E+1 3.45E-3
RWD [kg] 3.76E-3 8.26E-6 4.50E-4 0.00E+0 0.00E+0 0.00E+0 0.00E+0 2.60E-5 7.13E-7 0.00E+0 5.20E-5 3.49E-5
CRU [kg] 0.00E+0 0.00E+0 0.00E+0 0.00E+0 0.00E+0 0.00E+0 0.00E+0 0.00E+0 0.00E+0 0.00E+0 0.00E+0 0.00E+0
MFR [kg] 0.00E+0 0.00E+0 2.03E-2 0.00E+0 0.00E+0 0.00E+0 0.00E+0 0.00E+0 0.00E+0 1.00E-1 0.00E+0 0.00E+0
MER [kg] 0.00E+0 0.00E+0 0.00E+0 0.00E+0 0.00E+0 0.00E+0 0.00E+0 0.00E+0 0.00E+0 0.00E+0 0.00E+0 0.00E+0
EEE [MJ] 0.00E+0 0.00E+0 0.00E+0 0.00E+0 0.00E+0 0.00E+0 0.00E+0 0.00E+0 0.00E+0 0.00E+0 0.00E+0 0.00E+0
EET [MJ] 0.00E+0 0.00E+0 0.00E+0 0.00E+0 0.00E+0 0.00E+0 0.00E+0 0.00E+0 0.00E+0 0.00E+0 0.00E+0 0.00E+0
HWD = Hazardous waste disposed; NHWD = Non-hazardous waste disposed; RWD = Radioactive waste disposed; CRU = Components
Caption for re-use; MFR = Materials for recycling; MER = Materials for energy recovery; EEE = Exported electrical energy; EEE = Exported
thermal energy
6. LCA: Interpretation
Looking at the overall lifecycle, for most of the impact For ADPe, the use of the stainless steel screws in A5
categories (except for ADPe, EP and ODP), the contributes most significantly to the results. The EP is
manufacturing (A1-A3) of Hydropanel contributes to also strongly influenced by the landfilling of the
the largest share (> ~ 50 %) to the environmental cellulose-containing materials. The powder mix finisher
performance. contributes most significantly to the ODP of module
A5.
Within modules A1-A3, the pre-chains of the raw Interpretation of LCA-results in A1:
material have the most important impact (contribution The LCA for Hydropanel is mainly determined by the
> 50%) followed by the energy consumption for the pre-chains of the following raw materials: cement,
production. Transport to site (A2) has a negligible cellulose and silica sand flour. The contribution per
influence on the overall LCA results (contribution < impact category varies within these raw materials.
2.5%). Cement is most important for GWP, POCP and ADPe,
whereas cellulose has a significant impact on AP and
The re-emission of organic CO2 inherent in packaging EP. Compared to cement and cellulose, the
materials (wooden pallets, cardboards) as well as in contribution of silica sand is lower in all impact
cellulose takes place in module A5, in which the categories and only shows a relevant impact for ODP
packaging and the installation wastes are incinerated. (contribution >25%).
7. Requisite evidence
 At 5.6 μg/m³, the total VOC ("TVOC") after 3
7.1 Radioactivity days was below the limit of 10 mg/m³.
Radioactivity measurements confirm that no other
 At < 5 μg/m³, the total VOC ("TVOC") after 28
gamma emitters than those originating from the natural
days was below the limit of 1 mg/m³.
radiation sources are contained. The measured
radioactivity levels do not exceed the activity  At < 5 μg/m³, total SVOC after 28 days was
concentration indices as specified by the /Article 3 below the limit value of 0.1 mg/m³.
(Radiation Protection 112) for building products/  At > 5 μg/m³, the VOC individual substances
following the /Council Directive 96/29/. established after 28 days resulted in a rating
value R below the maximum limit of 1.
/Report on Radioactivity/
 At < 5 μg/m³, total individual VOC substances
7.2 Leaching without LCI value after 28 days were below
Leaching tests based on /EN 12457-2/ showed that no the limit value of 0.1 mg/m³
hazardous compounds were leached out.  At < 3 μg/m³, the formaldehyde concentration
after 28 days was below the limit of 120
/Report on Leaching/
μg/m³.
7.3 VOC emissions
/Report on VOC emissions/ The Hydropanel product under review is suitable for
use in interior applications in accordance with /AgBB/
Process: Testing the product emissions in accordance "Health-related Evaluation Procedure for Volatile
with the "Ausschuss zur gesundheitlichen Bewertung Organic Compounds Emissions (VOC and SVOC)
von Bauprodukten" (/AgBB/) method from Construction Products" in the version dated May
2010.
Results:
 Carcinogens were not detected after 3 and 28
days.
8. References
/Article 3 (Radiation Protection 112) for building https://www.nachhaltigesbauen.de/baustoff-und-
products/ gebaeudedaten/nutzungsdauern-von-bauteilen.html
Radiological Protection Principles concerning the
Natural Radioactivity of Building Materials, published in /Construction Products Regulation/
1999 by the Directorate-General Environment, Nuclear Regulation (EU) No 305/2011 of the European
Safety and Civil Protection Parliament and of the Council of 9 March 2011 laying
down harmonised conditions for the marketing of
/AgBB/ construction products and repealing Council Directive
Ausschuss zur gesundheitlichen Bewertung von 89/106/ EEC Text with EEA relevance
Bauprodukten, AgBB (engl. German Committee
for Health-Related Evaluation of Building Products) /Council Directive 96/29/
/Council Directive 96/29/Euratom/ of 13 May 1996
/BAM/ laying down basic safety standards for the protection of
Material Testing Institute of the state of the health of workers and the general public against
Brandenburg/Berlin and the German Federal Institute the dangers arising from ionizing radiation
for Materials Research and Testing
/DIN 4102-1/
/BBSR/ DIN 4102-1:1998, Fire behaviour of building materials
BBSR table "Service lives of components for life cycle and elements - Classification of building materials -
assessment according to Bewertungssystem Requirements and testing
Nachhaltiges Bauen (BNB)" Sustainable Building
Information Portal by the Federal Ministry of Transport, /DIN 53436/
Building and Urban Affairs (Bundesinstitut für Bau-, DIN 53436-1:2015-12, Generation of thermal
Stadt- und Raumforschung, BBSR) decomposition products from materials for their
8 Environmental Product Declaration ETEX – Hydropanel Fibre-Cement Drywall Panels
analytic-toxicological testing - Part 1: Decomposition Regulation (EU) No 528/2012 of the European
apparatus and determination of test temperature Parliament and of the Council of 22 May 2012
concerning the making available on the market and
/EN 12457-2/ use of biocidal products
NF EN 12457-2, December 2002, Characterization of
waste - Leaching - Compliance test for leaching of /PCR Part A/
granular waste materials and sludges - Part 2: one PCR Part A, Calculation rules for the LCA and
stage batch test at a liquid to solid ratio of 10 l/kg for requirements on the Background Report, Version 1.7,
materials with particle size below 4 mm (without or with Institut Bauen und Umwelt e.V., www.ibu-epd.com,
size reduction) 2018
/EN 12467/ /PCR Part B/
NF EN 12467, November 2012, Fibre-cement flat PCR Part B, Requirements on the EPD for Fibre
sheets - Product specification and test methods cement / Fibre concrete, Version 1.6, Institut Bauen
und Umwelt e.V., www.bau-umwelt.com, 2017
/EN 13501-1/
NF EN 13501-1+A1 February 2013, Fire classification /REACH Regulation/
of construction products and building elements - Part Regulation (EU) No 1907/2006 of the
1: classification using data from reaction to fire tests European Parliament and of the Council of 18
December 2006 concerning the Registration,
/EN 197-1/ Evaluation, Authorisation and Restriction of Chemicals
DIN EN 197-1:2011-11, Cement – Part 1: Composition, (REACH), establishing a European Chemicals Agency,
specifications and conformity criteria for common amending Directive 1999/45/EC and repealing Council
cement; German version EN 197-1:2011 Regulation (EEC) No 793/93 and Commission
Regulation (EC) No 1488/94 as well as Council
/Eurofins Analyses pour l’Environnement/ Directive 76/769/EEC and Commission Directives
Eurofins Analyses pour l'Environnement France 91/155/EEC, 93/67/EEC, 93/105/EC and 2000/21/EC
5, rue d'Otterswiller
67700, Saverne /Report on Radioactivity/
France Date: 2 December 2011
Measuring agency: /SCK.CEN Laboratory for
/Eurofins Product Testing A/S/ Gammaspectrometry/, Mol, Belgium
Smedeskovvej 38 Protocol: Activity concentration index (ACI)[AR1]
DK - 8464
Galten /Report on Leaching/
Denmark Date: 26 June 2015
Measuring agency: /Eurofins Analyses pour
/European Waste Index/ l’Environnement/ France-Site de Saverne[AR2]
European Waste Index provides an EU-wide common
terminology for waste classification. The index is in the /Report on VOC emissions/
Commission Decision of 3 May 2000 Date: 29.11.2011
Measuring agency: /Eurofins Product Testing A/S/
/GaBi documentation/ Smedeskovvej 38, 8464 Galten, Denmark;
GaBi 8.7 data set documentation for the software Report no. G10208A
system and data bases, LBP, University of Stuttgart
and thinkstep AG, Leinfelden-Echterdingen, 2018 /SCK.CEN Laboratory for Gamma spectrometry/
(http://www.gabi- SCK•CEN Research Center MolBoeretang 200
software.com/international/support/gabi/gabi-database- 2400 Mol
2018-lci-documentation) België
/GaBi ts software/ /Z-31.4-160/
GaBi Software-System and Database for Life General technical approval no. Z-31.4-160 of the
Cycle Engineering, 1992-2018, thinkstep AG, "Deutsches Institut für Bautechnik" (DIBt) for Eternit
Leinfelden-Echterdingen, with acknowledgement of facade panels
LBP University of Stuttgart, program version 8.7
/IBU 2016/
/ISO 9001/ IBU (2016): General Programme Instructions for the
UNI EN ISO 9001:2015 September 2015, Quality Preparation of EPDs at the Institut Bauen und Umwelt
management systems - Requirements e.V., Version 1.1 Institut Bauen und Umwelt e.V.,
Berlin.
www.ibu-epd.de
/ISO 14001/
UNI EN ISO 14001:2015, Environmental management /ISO 14025/
systems - Requirements with guidance for use DIN EN /ISO 14025:2011-10/, Environmental labels
and declarations — Type III environmental
/OHSAS 18001/ declarations — Principles and procedures
OHSAS 18001:2007, Occupational Health and Safety
Management Certification /EN 15804/
/EN 15804:2012-04+A1 2013/, Sustainability of
/Ordinance on Biocide Products/ construction works — Environmental Product
9 Environmental Product Declaration ETEX – Hydropanel Fibre-Cement Drywall Panels
Declarations — Core rules for the product category of
construction products
10 Environmental Product Declaration ETEX – Hydropanel Fibre-Cement Drywall Panels
Publisher
Institut Bauen und Umwelt e.V. Tel +49 (0)30 3087748- 0
Panoramastr. 1 Fax +49 (0)30 3087748- 29
10178 Berlin Mail info@ibu-epd.com
Germany Web www.ibu-epd.com
Programme holder
Institut Bauen und Umwelt e.V. Tel +49 (0)30 - 3087748- 0
Panoramastr 1 Fax +49 (0)30 – 3087748 - 29
10178 Berlin Mail info@ibu-epd.com
Germany Web www.ibu-epd.com
Author of the Life Cycle
Assessment Tel +49 711 341817-0
thinkstep AG Fax +49 711 341817-25
Hauptstraße 111- 113 Mail info@thinkstep.com
70771 Leinfelden-Echterdingen Web http://www.thinkstep.com
Germany
Owner of the Declaration
Etex Building Performance Tel +32 2 778 12 11
International Fax +32 2 778 12 12
Marcel Demonque 500 r Mail info@etexgroup.com
84915 Avignon Cedex 9 Web http://www.etexgroup.com
France
