ENVIRONMENTAL PRODUCT DECLARATION
as per ISO 14025 and EN 15804+A2
Owner of the Declaration Hilti Aktiengesellschaft
Publisher Institut Bauen und Umwelt e.V. (IBU)
Programme holder Institut Bauen und Umwelt e.V. (IBU)
Declaration number EPD-HIL-20230212-IBC2-EN
Issue date 01.09.2023
Valid to 31.08.2028
MT- System (Indoor)
HILTI AG
www.ibu-epd.com | https://epd-online.com
1. General Information
HILTI AG MT- System (Indoor)
Programme holder Owner of the declaration
IBU – Institut Bauen und Umwelt e.V. Hilti Aktiengesellschaft
Hegelplatz 1 Feldkircher Strasse 100
10117 Berlin 9494 Schaan
Germany Liechtenstein
Declaration number Declared product / declared unit
EPD-HIL-20230212-IBC2-EN I.-Channel MT-40D / 1kg
This declaration is based on the product category rules: Scope:
Connection, assembly and installation systems, 01.08.2021 This document relates to the I.-Channel MT-40D ('MT-40D”) as a
(PCR checked and approved by the SVR) representative product for the MT Indoor profile portfolio. The MT Indoor
profile portfolio is a set of installation channels with 5 types of wall
thickness – 1.2mm, 1.5mm, 1.75mm, 2mm and 2.75mm. Then the
Issue date products are distinguished into size classes by shape and load
performance. Each of these size classes are produced in 3 different
01.09.2023
lengths to accommodate intended use, which are 2 meters, 3 meters and 6
meters. The declared product for this EPD is MT-40D, with thickness of
2mm, because it is has the highest weight in the MT Indoor profile portfolio
Valid to
and therefore represents the worst case.
31.08.2028 The owner of the declaration shall be liable for the underlying information
and evidence; the IBU shall not be liable with respect to manufacturer
information, life cycle assessment data and evidences.
The EPD was created according to the specifications of EN 15804+A2. In
the following, the standard will be simplified as EN 15804.
Verification
The standard EN 15804 serves as the core PCR
Independent verification of the declaration and data according to ISO
14025:2011
Dipl.-Ing. Hans Peters internally X externally
(Chairman of Institut Bauen und Umwelt e.V.)
Florian Pronold Mrs Kim Allbury,
(Managing Director Institut Bauen und Umwelt e.V.) (Independent verifier)
1 Environmental Product Declaration - HILTI AG - MT- System (Indoor)
2. Product
2.1 Product description/Product definition
The MT-40 D is designed as a metallic substructure system that
is made of thin-walled steel in C shape with surface coating for
the indoor environment. The open side of the profile interfaces
with other assembly components to form a flexible modular
support substructure that is fastened to concreate or steel
frame structures. They are horizontal and vertical members at
different lengths that interconnect to form either 2D or 3D
structures to carry the weight and hold in place mechanical,
electrical, and piping services.
For the placing of the product on the market in the European
Union European Free Trade Association
EU/EFTA) (with the exception of Switzerland) Regulation (EU)
No. 305/2011 (CPR) applies. The product needs a declaration
of performance taking into consideration the following
European Technical Approval ETA-21/0414 assessed based on
EAD 280016-00-0602 'Products for installation systems for
supporting technical building equipment'. For the application
and use the respective national provisions apply.
The individual channel items under this product family and
represented by MT-40D are as listed below:
2 Environmental Product Declaration - HILTI AG - MT- System (Indoor)
2.2 Application
The MT-40D is developed to be fixed on base materials like
concrete and steel frame structures to support the mechanical,
electrical, and piping services so that their loads are transferred
to the super structure of the building or facility. The product is
intended to be used under dry indoor conditions for support:
- Pipes for the transport of fluids and gas
- Technical building equipment in general
- Components of fixed fire-fighting systems
- Electrical cable layouts
- Ventilating system layouts and equipment
- Flooring
- Other instrumentation
The profile flanges are turned at the end which makes it
possible to force-fit the channels to specific channel system
fixtures. Recesses in the form of oblong holes and round holes
allow the use of fasteners and fixtures.
2.3 Technical Data
The following data complies with the dimension drawing
provided in the Annexe A3 of ETA-21/0414.
Constructional data
Name Value Unit
Thickness of material 2 mm
Height of profile 85 mm
Width of profile 42.5 mm
Length of profile 6000.0 mm
Performance data of the product in accordance with the
declaration of performance with respect to its essential
characteristics according to ETA-21/0414 assessed based on
EAD 280016-00-0602 'Products for installation systems for
supporting technical building equipment'
2.4 Delivery status
The MT-40D is packaged in bundles of long goods, and each
length types are bundled together with plastic straps then
protected at the edges with wooden blocks. The declared MT-
40D is packed in 25 piece-bundle of 6 meter lengths,
constituting 150 meters per bundle in a delivery.
2.5 Base materials/Ancillary materials
Name Value Unit
Galvanized steel 100 %
3 Environmental Product Declaration - HILTI AG - MT- System (Indoor)
The raw material used to produce the declared product MT-40D meters in lengths. Same length types are bundled together in
is galvanized steel according to the standard EN 10346:2015, plastic straps (PE) and delivered on wooden blocks that protect
weighing 2.039 kg per meter. the ends of the bundles. Depending on the usage case and
user request, the channel can be cut into various lengths as
This product/article/at least one partial article contains requested and bundled or preassembled in customized
substances listed in the REACH SVHC candidate list (date: conditions.
17.01.2023) exceeding 0.1 percentage by mass: NO. Both materials cannot be re-used, but they can be recycled.
The PE plastic straps can be collected per recycle waste
This product/article/at least one partial article contains other collection process and can be recycled through thermal
carcinogenic, mutagenic, reprotoxic (CMR) substances in recycling method.
categories 1A or 1B which are not on the candidate list,
exceeding 0.1 percentage by mass: NO. 2.10 Condition of use
All supplied materials are protected in the installed condition
Biocide products were added to this construction product or it against external influences and designed for the service life of
has been treated with biocide products (this then concerns a the respective construction. No risks can arise to water, air and
treated product as defined by the (EU) Ordinance on Biocide soil if the products are used as designated in an indoor dry
Products No. 528/2012): NO. environment.
2.6 Manufacture 2.11 Environment and health during use
The raw material for MT-40D is sourced from Linz, Austria and When used as designated, there is no impact on the
transported to Gresten, Austria via train. The profile is environment or health.
manufactured through cold-roll forming process of steel sheets
2.12 Reference service life
which also includes cutting to designated lengths at the end of
the line. The MT-40D has an assumed service life of 50 years in
accordance with the BBSR table 'Service lives of Components
for life cycle assessment according to BNB'. The practical
service life can however be considerably longer and will
depend on the specific installation situation and the product
exposure scenario. The main factors influencing the period of
use involve weathering as well as mechanical loads.
2.13 Extraordinary effects
Fire
The MT-40D is assessed in accordance with the European
2.7 Environment and health during manufacturing Assessment Document EAD 280016-00-0502 for the following
Hilti ensures that the suppliers implement a quality performance in safety in case of fire (BWR2).
management system that meets the requirements of the ISO Fire protection
9001 or ISO/TS 16949 standards or higher. Quality must be
Name Value
planned, ensured and documented using appropriate quality
Reaction to fire Class A1
tools, e.g. Statistical process contro (SPC) or failure mode and
effects analysis (FMEA). The production and quality control Pull-through resistance of channel back holes ETA
according to the product specifications and approval under fire exposure 23/0105
specifications of the MT profile and its system components are ETA
Bending characteristics under fire exposure
ensured by an in-house quality control by Hilti. 23/0105
We expect the environmental management implemented by our
suppliers to meet at least the ISO14001 standard international
Water
regulations on forbidden substances.
The MT-40D is comprised of galvanized steel. There are no
environmental risks attributable to the effects of water except
The supplier for the MT-40D holds the following certifications:
the product's own corrosion impact.
- ISO 9001
- ISO 45001
Mechanical destruction
- ISO 14001
In the event of mechanical destruction of the MT-40D, the
profile assembly has to be replaced with a new set for the
2.8 Product processing/Installation
intended functional performance.
The MT-40D is supplied as a ready to install modular support
system element provided with an Instruction for Use explaining 2.14 Re-use phase
the basic steps for installation. The MT-40D is either connected
The MT-40D cannot be re-used as a component for a modular
to a pre-positioned baseplate element that connects it to the
support system, but the material can be recycled. All
building structure or is positioned directly to the building
components of the described product can be returned and
structure when delivered as a pre-assembled module. For
recycled into the material cycle.
fastening the connection point to the baseplate or other
connection elements, a Hilti automated impact wrench tool 2.15 Disposal
called SIW 6AT-A22 may be used to ensure anchoring or The MT-40D is disassembled from a building in which it has
bolting at precise fastening torques. No special environmental been installed by a series of unfastening processes. The
protection measures need to be taken while installing the MT interfaces with assembly components and with concrete or
profiles. steel structures which have been originally fastened with a bolt
and nut mechanism are untightened and separated back into
2.9 Packaging
individual product parts without change or deformation of the
The MT-40D is delivered packed and strapped in bundles as
product material. These are fed into the recycling process in
long goods. The product type can be 2 meters, 3 meters or 6
accordance with the applicable disposal guidelines. The waste
4 Environmental Product Declaration - HILTI AG - MT- System (Indoor)
code for the profiles in accordance with the European Waste Further information is available on the Hilti website:
Index is 17 04 05 (iron and steel). www.hilti.group
2.16 Further information
3. LCA: Calculation rules
3.1 Declared Unit
The declared product here is a mounting system from HILTI AG
with the designation I. Channel MT-40D is a representative
product of the MT Indoor portfolio. The declared unit refers to 1
kg of mounting system. The packaging, related to 1 kg of
Illustration 2: Information module A1 to A3 of packaging
mounting rail, is additionally included in the calculation at 0.007
kg. The following table shows the data of the declared unit.
In the information modules C1 to C4, the deconstruction or
Declared unit and mass reference demolition from the building, the transport to waste disposal,
Name Value Unit the waste treatment and disposal of the product are recorded.
Furthermore, reuse, recovery and recycling potentials are
Declared unit 1 kg
reported in information module D.
Declared unit 7850 kg/m3
Mass reference 4,46 kg/m 3.3 Estimates and assumptions
conversion factor 4,46 A steel coil with zinc content was used for the MT-40D. The
transport of the lubricant was not taken into account, as the
mass fraction is small and the effect is estimated to be low.
3.4 Cut-off criteria
The transport for the lubricant was not taken into account as
3.2 System boundary
the mass fraction is small. The lubricant itself was taken into
Type of EPD: Cradle to factory gate with options. The following
account in the production for transparency of production.
information modules are defined as system boundaries in this
The cut-off criterion according to EN 15804+A2 is otherwise not
study:
applied. All energy and mass inputs were taken into account.
3.5 Background data
Production stage (A1- A3): The background data referred to in this study comes from
- A1, raw material extraction, Sphera's LCA for Experts database.
- A2, transport to the manufacturer,
- A3, production. 3.6 Data quality
For the preparation of the LCA, specific data from the Gersten
plant in Austria of HILTI AG from the year 2022 were collected.
End of life (C1- C4): The background data from the LCA for Experts database is
- C1, deconstruction/demolition, from 2023 and therefore highly relevant.
- C2, transport, The data quality is rated as adequate.
- C3, waste treatment ,
- C4, disposal. 3.7 Period under review
The input and output flows used in this calculation come from
the annual average consumption from the year 2022.
Reuse, recovery and recycling potential (D).
3.8 Geographic Representativeness
Land or region, in which the declared product system is
In order to accurately capture the indicators and environmental manufactured, used or handled at the end of the product´s
impacts of the declared unit, a total of 8 information modules lifespan: Global
are considered. The information modules A1 to A3 describe the
material provision, the transport to the production site, as well
3.9 Allocation
as the production processes of the product itself.
The I.Channel MT-40D assembly system as a representative
product of the MT Indoor portfolio is produced in Gresten,
Austria. The data for input and output flows are taken from the
The primary products are sourced from the European Union.
year 2022, which corresponds to the annual average. The input
The transport is carried out by lorry and train. The following flow
and output flows used in this calculation were measured directly
charts illustrate the underlying production process.
by the manufacturer for this production process and are shown
in the following table. In order to calculate the net flows, the
mass that is produced as production waste and used as
external steel scrap is subtracted from the total mass of
secondary material.
Illustration 1: Information module A1 to A3 of product
3.10 Comparability
Basically, a comparison or an evaluation of EPD data is only
possible if all the data sets to be compared were created
according to EN 15804 and the building context, respectively
the product-specific characteristics of performance, are taken
into account. The database referred to in this study is LCA for
5 Environmental Product Declaration - HILTI AG - MT- System (Indoor)
Experts by Sphera.
4. LCA: Scenarios and additional technical information
out with an electric screwdriver. The electrical energy
Characteristic product properties of biogenic carbon consumption for the tool is assumed to be 0.003 MJ for the
The declared product does not contain any biogenic specified unit. The electricity consumption is calculated with a
Carbon. German electricity mix.
Information on describing the biogenic Carbon Content at In information module C3, the waste treatment (sorting and
factory gate pressing) of the steel is calculated.
Name Value Unit Name Value Unit
Biogenic carbon content in accompanying kg Collected separately waste type waste type 1 kg
0.0018
packaging C Recycling 1 kg
Note: 1 kg of biogenic carbon is equivalent to 44/12 kg of CO .
2 Reuse, recovery and/or recycling potentials (D), relevant
scenario information
In Module D, a recycling rate of 85% is assumed (world steel
association).
End of life (C1-C4) Name Value Unit
In information module C1, the demolition of the mounting Recycling 0,85 kg
system from the building is calculated. The demolition is carried
6 Environmental Product Declaration - HILTI AG - MT- System (Indoor)
5. LCA: Results
DESCRIPTION OF THE SYSTEM BOUNDARY (X = INCLUDED IN LCA; MND = MODULE OR INDICATOR NOT DECLARED; MNR
= MODULE NOT RELEVANT)
Benefits and
Construction loads beyond
Product stage Use stage End of life stage
process stage the system
boundaries
la ire ta m w a Ry lp p u s tro p s n a rT g n iru tc a fu n a M e h t m o rf tro p s n a rTe tis e h t o t e ta g y lb m e s s A e s U e c n a n e tn ia M ria p e R tn e m e c a lp e R tn e m h s ib ru fe R y g re n e la n o ita re p Oe s u re ta w la n o ita re p Oe s u n o itc u rts n o c -e Dn o itilo m e d tro p s n a rT g n is s e c o rp e ts a W la s o p s iD -e s u e R-y re v o c e R-g n ilc y c e Rla itn e to p
A1 A2 A3 A4 A5 B1 B2 B3 B4 B5 B6 B7 C1 C2 C3 C4 D
X X X MND MND MND MND MNR MNR MNR MND MND X X X X X
RESULTS OF THE LCA - ENVIRONMENTAL IMPACT according to EN 15804+A2: 1 kg I.Channel MT-40D
Parameter Unit A1-A3 C1 C2 C3 C4 D
Global Warming Potential total (GWP-total) kg CO 2 eq 2.83E+00 7.28E-04 4.41E-03 1.69E-02 0 -1.89E+00
Global Warming Potential fossil fuels (GWP-fossil) kg CO 2 eq 2.83E+00 7.28E-04 4.39E-03 1.69E-02 0 -1.89E+00
Global Warming Potential biogenic (GWP-biogenic) kg CO 2 eq 1.64E-03 1.58E-07 0 4.11E-06 0 -1.02E-03
Global Warming Potential luluc (GWP-luluc) kg CO 2 eq 1.22E-03 1.06E-07 1.61E-05 2.12E-06 0 -6.72E-04
Depletion potential of the stratospheric ozone layer (ODP) kg CFC11 eq 2.15E-12 4.29E-17 7.63E-16 1.58E-10 0 -1.42E-12
Acidification potential of land and water (AP) mol H+ eq 6.53E-03 8.57E-07 1.69E-05 9.99E-05 0 -4.14E-03
Eutrophication potential aquatic freshwater (EP-freshwater) kg P eq 2.83E-06 7.24E-11 1.02E-08 3.05E-07 0 -1.44E-06
Eutrophication potential aquatic marine (EP-marine) kg N eq 1.65E-03 2.85E-07 8.07E-06 4.53E-05 0 -1.06E-03
Eutrophication potential terrestrial (EP-terrestrial) mol N eq 1.79E-02 3.1E-06 9.02E-05 4.92E-04 0 -1.14E-02
Formation potential of tropospheric ozone photochemical oxidants kg NMVOC
5.47E-03 7.87E-07 1.53E-05 1.45E-04 0 -3.5E-03
(POCP) eq
Abiotic depletion potential for non fossil resources (ADPE) kg Sb eq 1.13E-07 3.01E-12 3.09E-10 3.49E-09 0 -7.25E-08
Abiotic depletion potential for fossil resources (ADPF) MJ 3.77E+01 1.07E-02 5.92E-02 2.29E-01 0 -1.68E+01
m3 world eq
Water use (WDP) 3.43E-02 4.08E-06 2.27E-05 4.76E-04 0 -2.2E-02
deprived
RESULTS OF THE LCA - INDICATORS TO DESCRIBE RESOURCE USE according to EN 15804+A2: 1 kg I.Channel MT-40D
Parameter Unit A1-A3 C1 C2 C3 C4 D
Renewable primary energy as energy carrier (PERE) MJ 1.56E+00 4.08E-05 3.83E-03 1.12E-03 0 -9.97E-01
Renewable primary energy resources as material utilization
MJ 8E-02 0 0 0 0 0
(PERM)
Total use of renewable primary energy resources (PERT) MJ 1.64E+00 4.08E-05 3.83E-03 1.12E-03 0 -9.97E-01
Non renewable primary energy as energy carrier (PENRE) MJ 3.77E+01 1.07E-02 5.92E-02 2.29E-01 0 -1.69E+01
Non renewable primary energy as material utilization (PENRM) MJ 1.2E-01 0 0 0 0 0
Total use of non renewable primary energy resources (PENRT) MJ 3.79E+01 1.07E-02 5.92E-02 2.29E-01 0 -1.69E+01
Use of secondary material (SM) kg 1.98E-01 0 0 0 0 0
Use of renewable secondary fuels (RSF) MJ 0 0 0 0 0 0
Use of non renewable secondary fuels (NRSF) MJ 0 0 0 0 0 0
Use of net fresh water (FW) m3 1.67E-03 1.61E-06 3.48E-06 2.52E-05 0 -9.95E-04
RESULTS OF THE LCA – WASTE CATEGORIES AND OUTPUT FLOWS according to EN 15804+A2:
1 kg I.Channel MT-40D
Parameter Unit A1-A3 C1 C2 C3 C4 D
Hazardous waste disposed (HWD) kg 4.4E-10 5.45E-13 1.59E-13 5.05E-12 0 4.42E-11
Non hazardous waste disposed (NHWD) kg 3.08E-02 2.81E-06 8.63E-06 2.6E-05 0 -2.3E-02
Radioactive waste disposed (RWD) kg 1.88E-04 9.32E-07 6.19E-08 8.63E-06 0 -9.96E-05
Components for re-use (CRU) kg 0 0 0 0 0 0
Materials for recycling (MFR) kg 6.3E-03 0 0 8.5E-01 0 0
Materials for energy recovery (MER) kg 0 0 0 0 0 0
Exported electrical energy (EEE) MJ 0 0 0 0 0 0
Exported thermal energy (EET) MJ 0 0 0 0 0 0
RESULTS OF THE LCA – additional impact categories according to EN 15804+A2-optional:
1 kg I.Channel MT-40D
Parameter Unit A1-A3 C1 C2 C3 C4 D
Disease
Incidence of disease due to PM emissions (PM) ND ND ND ND ND ND
incidence
Human exposure efficiency relative to U235 (IR) kBq U235 eq ND ND ND ND ND ND
Comparative toxic unit for ecosystems (ETP-fw) CTUe ND ND ND ND ND ND
Comparative toxic unit for humans (carcinogenic) (HTP-c) CTUh ND ND ND ND ND ND
Comparative toxic unit for humans (noncarcinogenic) (HTP-nc) CTUh ND ND ND ND ND ND
7 Environmental Product Declaration - HILTI AG - MT- System (Indoor)
Soil quality index (SQP) SQP ND ND ND ND ND ND
Disclaimer 1 – for the indicator 'Potential Human exposure efficiency relative to U235'. This impact category deals mainly with the
eventual impact of low-dose ionizing radiation on human health of the nuclear fuel cycle. It does not consider effects due to possible
nuclear accidents, occupational exposure or radioactive waste disposal in underground facilities. Potential ionizing radiation the soil,
from radon and from some construction materials is also not measured by this indicator.
Disclaimer 2 – for the indicators 'abiotic depletion potential for non-fossil resources', 'abiotic depletion potential for fossil resources',
'water (user) deprivation potential, deprivation-weighted water consumption', 'potential comparative toxic unit for ecosystems', 'potential
comparative toxic unit for humans – cancerogenic', 'Potential comparative toxic unit for humans - not cancerogenic', 'potential soil
quality index'. The results of this environmental impact indicator shall be used with care as the uncertainties on these results are high
as there is limited experience with the indicator.
6. LCA: Interpretation
The dominance analysis shows that the main causes of
environmental impacts and indicators are to be found in
information module A1. This shows the total global warming The assembly system itself accounts for 98% of the total global
potential for material supply with approx. 55% and approx. 10% warming potential in information module A1. Approx. 2% is
for production, related to all information modules. accounted for by the plastic strap
Illustration: Dominance analysis A1- A3
Looking at the material supply of the assembly system and the
packaging in the de-tail, it becomes clear which raw materials Illustration: Dominance analysis A1
contribute decisively to the respective environmental impacts
and indicators.
7. Requisite evidence
The MT-40D may be used to constitute a supporting system to and cable ladder systems. Therefore, requisite evidence
carry the load of cable trays and ladders but is not within scope pertaining to this standard shall not be given for this product.
of the DIN EN 61537 which is specific to cable tray systems
8. References
Standards ISO 9001:2015
Quality management system
EN 10346:2015
Continuously hot-dip coated steel flat products for cold fo ming -
Technical delivery conditions ISO 14001:2015
Environmental Management System
EN 15804
EN 15804:2012+A1 2013, Sustainability of construction works
— Environmental Product Declarations — Core rules for the ISO 14025
product category of construction products. EN ISO 14025:2011, Environmental labels and declarations —
Type III environmental declarations — Principles and
EN 15804 procedures
EN 15804:2012+A2:2019+AC:2021, Sustainability of
construction works — Environmental Product Declarations — ISO 15686
Core rules for the product category of construction products. Buildings and constructed assets
EN 61537 ISO 45001:2018
DIN EN 61537 VDE 0639:2007-09 , Occupational health and safety system
Cable management
Cable tray systems and cable ladder systems Further references
(IEC 61537:2006); German version EN 61537:2007
Candidate List of substances of very high concern for
8 Environmental Product Declaration - HILTI AG - MT- System (Indoor)
Authorisation Environmental Product Declarations for Institut Bauen und
European Chemicals Agency (ECHA), in accordance with Umwelt (IBU), Part A: Calculation Rules for the Life Cycle
Article 50(10) of the REACH regulation Assessment and Requirements on the Project Report according
to EN 15804+A2:2019, 202108
European Technical Approval ETA-21/0414 Hilti Installation
channels of MT system PCR Part B
assessed based on EAD 280016-00-0602 'Products for Connection, assembly and installation systems,.10.2022
installation systems for supporting technical building equipment'
Regulation (EU) No. 305/2011 (CPR)
European Technical Approval ETA-23/0105 Regulation (EU) No 305/2011 of the European Parliament
andof the Council of 9 March 2011 laying down
harmonisedconditions for the marketing of construction
European Waste code products andrepealing Council Directive 89/106/EEC Text with
in accordance with the European Waste Catalogue (EWC) EEArelevance
(EWC 2014/955/EU) Commission Decision amending Decision
2000/532/EC on the list of waste pursuant to Directive Sphera
2008/98/EC of the European Parliament and of the Council LCA for Experts: Ganzheitliche Bilanzierung
Leinfelden-Echterdingen; Sphera Solution GmbH (Hrsg.)
http://www.gabi-software.com/deutsch/index/
IBU 2021
General Instructions for the EPD programme of Institut Bauen World steel association
und Umwelt e.V. Version 2.0, Berlin: Institut Bauen und Umwelt https://www.worldsteel.org/steel-topics/raw-materials/
e.V.,2021 www.ibu-epd.de
PCR Part A
Institut Bauen und Umwelt e.V, Berlin (pub.): Product Category
Rules for Construction Products from the range of
9 Environmental Product Declaration - HILTI AG - MT- System (Indoor)
Publisher
Institut Bauen und Umwelt e.V. +49 (0)30 3087748- 0
Hegelplatz 1 info@ibu-epd.com
10117 Berlin www.ibu-epd.com
Germany
Programme holder
Institut Bauen und Umwelt e.V. +49 (0)30 3087748- 0
Hegelplatz 1 info@ibu-epd.com
10117 Berlin www.ibu-epd.com
Germany
Author of the Life Cycle Assessment
FIT-Umwelttechnik GmbH 05362 72 69 474
Westerstr. 13 bertram@fit-umwelttechnik.de
38442 Wolfsburg www.fit-umwelttechnik.com
Germany
Owner of the Declaration
Hilti Aktiengesellschaft +423 234 2111
Feldkircher Strasse 100 HAGHSE@hilti.com
9494 Schaan www.hilti.com
Liechtenstein
10 Environmental Product Declaration - HILTI AG - MT- System (Indoor)
