ENVIRONMENTAL PRODUCT DECLARATION
as per ISO 14025 and EN 15804+A2
Owner of the Declaration Grundfos Holding A/S
Publisher Institut Bauen und Umwelt e.V. (IBU)
Programme holder Institut Bauen und Umwelt e.V. (IBU)
Declaration number EPD-GRU-20240273-CBA1-EN
Issue date 01/08/2024
Valid to 31/07/2029
MAGNA3 25,32-40/60/80/100/120, 32-40/60/80/100 F, 40-40/60 F
(Cast iron)
Grundfos Holding A/S
www.ibu-epd.com | https://epd-online.com
General Information
Grundfos Holding A/S MAGNA3 25,32-40/60/80/100/120, 32-40/60/80/100 F,
40-40/60 F (Cast iron)
Programme holder Owner of the declaration
IBU – Institut Bauen und Umwelt e.V. Grundfos Holding A/S
Hegelplatz 1 Poul Due Jensens Vej 7
10117 Berlin 8850 Bjerringbro
Germany Denmark
Declaration number Declared product / declared unit
EPD-GRU-20240273-CBA1-EN 1 PCS. of MAGNA3 (cast iron) pump
This declaration is based on the product category rules: Scope:
Pumps for liquids and liquids with solids, 01/08/2021 The declaration applies to 1 piece of MAGNA3 (Cast iron) pump.
(PCR checked and approved by the SVR)
The product is produced in Wahlstedt, Germany, and the life cycle
assessment is based on data collected at the production site. Production
Issue date has been modeled using annual production data from 2022.
The declaration covers the following MAGNA3 products with cast iron
01/08/2024
pump house:
MAGNA3 25-40/60/80/100/120 (threaded),
MAGNA3 32-40/60/80/100/120 (threaded),
Valid to
MAGNA3 32-40/60/80/100 F (flanged),
31/07/2029 MAGNA 3 40-40/60 F (flanged).
The owner of the declaration shall be liable for the underlying information
and evidence; the IBU shall not be liable with respect to manufacturer
information, life cycle assessment data and evidences.
The EPD was created according to the specifications of EN 15804+A2. In
the following, the standard will be simplified as EN 15804.
Verification
The standard EN 15804 serves as the core PCR
Independent verification of the declaration and data according to ISO
Dipl.-Ing. Hans Peters
14025:2011
(Chairman of Institut Bauen und Umwelt e.V.)
internally X externally
Florian Pronold Mrs Kim Allbury,
(Managing Director Institut Bauen und Umwelt e.V.) (Independent verifier)
1 Environmental Product Declaration - Grundfos Holding A/S - MAGNA3 25,32-40/60/80/100/120, 32-40/60/80/100 F, 40-40/60 F (Cast iron)
Product
· solar-heating systems
Product description/Product definition The pump is suitable for thin, clean, non-aggressive and non-
The Grundfos MAGNA3 circulator pumps are designed for explosive liquids, not containing solid particles or fibres that
circulating liquids in heating systems, air conditioning and may attack the pump mechanically or chemically. In heating
cooling systems and domestic hot water systems. However, the systems, the water must meet the requirements of accepted
pump range can also be used in ground source heat pump standards on water quality in heating systems. The pumps are
systems and solar heating systems. also suitable for domestic hot-water systems.
The MAGNA3 pump is a centrifugal pump powered by an
electrical motor. It has a high-performance neodymium magnet Technical Data
rotor which increases motor efficiency and an insulation shell to The performance data of the product according to the
reduce heat loss from the cast iron pump housing with threaded harmonized norms, based on the harmonization provisions
or flanged connections. above apply.
The relevant technical specifications according to the PCR Part
The declaration represents a weighted average of MAGNA3 B are given in the table below.
pumps with identical control box and motor/pump head. The Characteristics that are the same for all product groups are only
size of the pump housing distinguishes the different pumps, given once. Others are given individually for all products.
indicated in the first numbers: 25 (threaded), 32 (threaded), 32
F (flanged), 40 F (flanged). The average is defined based on
Constructional data
sales volumes.
Name Value Unit
Materials as well as supply chain and manufacturing processes
are identical, i.e., all cradle to gate processes (A1-A3). The Frequency 50 / 60 Hz
packaging is the high runner type for the included products. Voltage 230 V
The products are also identical in terms of distribution, Pumped liquid water -
reference service life and end-of-life treatment.
Energy Efficiency Index (all, except 40-60 F) 0,18
Another thing that differentiates the products from each other is
Energy Efficiency Index (40-60 F) 0,19
the software which controls how the pump operates in the
system in which it is installed, making them fit for different Head max. (25,32-40, 32,40-40 F) 4 m
applications. This is indicated in the second numbers: 40, 60, Head max. (25,,32-60, 32,40-60 F) 6 m
80, 100, 120. Hence, the use stage module B6 will change, as Head max. (25,32-80, 32-80 F) 8 m
the applied scenarios for electricity consumption changes.
Head max. (25,32-100, 32-100 F) 10 m
Head max. (25,32-120) 12 m
Flow range max (25-40) 6,5 m3/h
For the placing on the market in the European Union/European Flow range max (25-60) 8,7 m3/h
Free Trade Association (EU/EFTA) (with the exception of Flow range max (25-80) 10,3 m3/h
Switzerland) the following legal provisions apply:
Flow range max (25-100) 11 m3/h
Machinery Directive (2006/42/EC):
Standard used: EN 809:1998 + A1:2009 Flow range max (25-120) 12,5 m3/h
Radio Equipment Directive (2014/53/EU) Flow range max (32-40, 32-40 F) 8 m3/h
Standards used:
Flow range max (32-60, 32-60 F) 10 m3/h
EN 60335-1:2012+AC:2014+A11:2014+A13:2017+A1:2019
+A14:2019+A2:2019+A15:2021, EN 60335-2-51:2003 + Flow range max (32-80, 32-80 F) 11,3 m3/h
A1:2008 + A2:2012, EN 62233:2008. EN 55014-1:2006 + Flow range max (32-100, 32-100 F) 12,3 m3/h
A1:2009 + A2:2011, EN 55014-1:2017, EN 61000-6-2:2005, EN Flow range max (32-120) 12,6 m3/h
61000-3-2:2014, EN 61000-3-3:2013, ETSI EN 301 489-1
Flow range max (40-40 F) 13 m3/h
V2.2.0, ETSI EN 301 489-17 V3.2.0. ETSI EN 300 328 V2.1.1
Ecodesign Directive (2009/125/EC) Flow range max (40-60 F) 17,4 m3/h
Commission Regulation (EC) No 641/2009 and Commission Nominal capacity (25-40) 0,05 kW
Regulation (EC) No 622/2012
Nominal capacity (25-60) 0,084 kW
Standards used: EN 16297-1:2012, EN 16297-2:2012
Nominal capacity (25-80) 0,116 kW
RoHS Directive 2011/65/EU and 2015/863//EU
Standard: EN IEC 63000:2018 Nominal capacity (25-100) 0,153 kW
Nominal capacity (25-120) 0,185 kW
The CE marking takes into account the proof of conformity with Nominal capacity (32-40, 32-40 F) 0,068 kW
the respective harmonized norms based on the legal provisions
Nominal capacity (32-60, 32-60 F) 0,103 kW
above.
Nominal capacity (32-80, 32-80 F) 0,136 kW
MAGNA3 pumps are not harmonized in accordance with the
Nominal capacity (32-100, 32-100 F) 0,171 kW
CPR.
Nominal capacity (32-120) 0,182 kW
Application
Nominal capacity (40-40 F) 0,098 kW
For the application and use the respective national provisions
Nominal capacity (40-60 F) 0,185 kW
apply.
The pump is designed for circulating liquids in the following Average power input values are declared in Chapter 4. LCA
systems: Scenarios, see table "Operational energy use (B6)".
· heating systems
· air-conditioning and cooling systems Performance data of the product according to the harmonised
· ground-source heat-pump systems standards, based on provisions for harmonisation.
2 Environmental Product Declaration - Grundfos Holding A/S - MAGNA3 25,32-40/60/80/100/120, 32-40/60/80/100 F, 40-40/60 F (Cast iron)
Base materials/Ancillary materials The Wahlstedt production has been assessed and certified as
Name Value Unit meeting the requirements in ISO 14001, ISO 50001, ISO 45001
Aluminium 5,6 % and ISO 9001.
Ceramics 0,8 %
Reference service life
Copper 3,6 %
No use stage scenario which refers to the lifetime of the product
Magnet Nd 2.0 % is declared. However, to facilitate building calculations, an
Paper 3,7 % estimated RSL of 10 years can be used. This is an EU
PCB 4,9 % consensus-based estimation, referenced on page 37 in
Appendix 7: Lot 11 – Circulators in Buildings, prepared by AEA
Plastics 0,5 %
Energy & Environment for the European Commission in the
Plastics, foam 1,5 %
context of the Eco Design Directive:
Plastics GF 12,6 %
Rubber 0,3 % There is no definitive information on the average circulator life
Stainless steel 7.0 % available, there is consensus within the industry that it is at
least 12 years. However, this is complicated by many factors,
Steel 7,1 %
including many being scrapped prematurely when e.g. the
Cast iron 43,7 %
boiler they are connected to is replaced.
Cardboard 6,7 %
Plastic film 0,03 % From the estimated stock (140Mpa) and annual sales (14Mpa),
TOTAL 100 % the average lifetime of the circulator is taken as 10 years for the
purposes of this study.
The RSL of the declared product is not directly influencing the
REACH
results in this study, as no declared use stage scenario is
dependent on the RSL; The use stage sub-module B6 is
This product/article contains substances listed in the ECHA
declared per year as required by the PCR Part B.
candidate list (date: 10.06.2022) exceeding 0.1 percentage by
mass: no
LCA: Calculation rules
to the regional distribution centre, and finally to the construction
Declared Unit and product application site. Module A5 refers to the installation
The declared unit is 1 piece (pcs.) of MAGNA3 (Cast iron) process of the pump including the transportation of packaging
pump. waste to the treatment site and the waste treatment of
Declared unit packaging. The use of energy during installation is negligible for
the selected functional unit.
Mass includes packaging.
Name Value Unit
Use stage (B1-B7):
Declared unit 1 pce. In this study, all use stage modules are assessed, though B1,
Mass reference 6.1 kg/pce B2 and B7 are assessed to be zero. By decision no. 20170712-
Conversion factor [Mass/Declared Unit] 6.1 n of the SVR, the modules B3, B4 and B5 are by default
declared as "MNR" (module not relevant).
Other declared units are allowed if the conversion is shown
Contributions to operational energy use during the use stage
transparently.
(B6) come from the electricity consumption of the product. The
annual electricity consumption is calculated by multiplying the
The weighted average product has been calculated based on
average power input, which is based on a defined load profile,
the sales volumes of the included product models.
with the annual running hours. For use stage (B6) European
Average electricity grid mix has been used. These values are
System boundary
declared in the scenarios section.
This EPD is Cradle-To-Grave and Module D. The system
boundaries of the EPD follow the modular approach in EN
The End-of-Life stage (C1-C4)
15804.
The End-of-Life stage (C1-C4) Modules C1-C4 refer to the End-
of-life stage. A product reaches the end-of-life of its service life
Production and installation (A1-A5)
when it no longer provides any functionality. This life cycle
Modules A1-A3 refer to the product stage and includes raw
stage includes all activities from the end-of-life of the control
materials extraction and processing, transportation, and the
valve until all materials and components are processed, reused,
manufacturing process. The product stage is included in this
recycled, or disposed of.C1 regards the dismantling of the
study, and according to EN 15804:2019 + A2 the system
pump, and this module is a manual activity. C2 regards the
boundary with nature is set to include those processes that
transport to waste processing, C3 refers to the processing
provide the material and energy inputs into the system and the
(shredding) of waste for recycling, and C4 refers to waste
following manufacturing, transport up to the factory gate as well
disposal: landfilling and incineration. The End-of-Life
as the processing of waste arising from those processes. The
assumption is that 95 % is collected as electronic waste, while
assembly of the product, as well as the packaging, are also
5 % goes to landfill. The specific amounts are shown in the
included in A1-A3. Wastes and losses are included in the
scenarios section.
modules where they occur according to the polluter pays
principle and the modular approach of EN 15804:2019+A2
Beyond system boundary (D):
Module D refers to the burdens and benefits beyond the system
Module A4 regards the transportation from the production site
3 Environmental Product Declaration - Grundfos Holding A/S - MAGNA3 25,32-40/60/80/100/120, 32-40/60/80/100 F, 40-40/60 F (Cast iron)
boundaries. According to EN15804:A2+2019, module D manufactured, used or handled at the end of the product´s
includes the reuse, recovery and/or recycling potentials, lifespan: Europe
expressed in net impacts and benefits. Contributions to module
D come from waste incineration processes in A5 and C4 as well
Comparability
as material (metal) recycling in C3. The specific fractions and
net flows are shown in the scenarios section. Basically, a comparison or an evaluation of EPD data is only
possible if all the data sets to be compared were created
according to EN 15804 and the building context, respectively
the product-specific characteristics of performance, are taken
Geographic Representativeness into account. The primary database used for background data
Land or region, in which the declared product system is is Sphera, while Ecoinvent served as a secondary database.
LCA: Scenarios and additional technical information
Name Value Unit
Characteristic product properties of biogenic carbon
Electricity consumption 25-40 114 kWh/a
The biogenic carbon content quantifies the amount of biogenic
Electricity consumption 25-60 192 kWh/a
carbon in a construction product leaving the factory gate, and it
will be separately declared for the product and for any Electricity consumption 25-80 265 kWh/a
accompanying packaging, as required from the PCR Part A. Electricity consumption 25-100 350 kWh/a
The carbon content of cardboard and paper is assumed to 0.43 Electricity consumption 25-120 423 kWh/a
kg C, meaning 43% of the paper and cardboard packaging is
Electricity consumption 32-40, 32-40 F 156 kWh/a
biogenic carbon. Overall, there is an amount of weight-%
Electricity consumption 32-60, 32-60 F 236 kWh/a
Carbon in the product leaving the factory gate and has to be
considered Electricity consumption 32-80, 32-80 F 311 kWh/a
Electricity consumption 32-100, 32-100 F 391 kWh/a
Information on describing the biogenic Carbon Content at Electricity consumption 32-120 416 kWh/a
factory gate Electricity consumption 40-40 F 224 kWh/a
Name ValueUnit Electricity consumption 40-60 F 423 kWh/a
Biogenic carbon content in accompanying kg Running hours (all products) 5.000 h/a
0.273
packaging C Average power input, 25-40 0,023 kW
Note: 1 kg of biogenic carbon is equivalent to 44/12 kg of CO2 Average power input 25-60 0,038 kW
Average power input 25-80 0,053 kW
Average power input 25-100 0,070 kW
Average power input 25-120 0,085 kW
Transport from the gate to the site (A4)
Average power input 32-40, 32-40 F 0,031 kW
Name Value Unit Average power input 32-60, 32-60 F 0,047 kW
Litres of fuel 1,7 l/100 tkm Average power input 32-80, 32-80 F 0,062 kW
Transport distance 1513 km Average power input 32-100, 32-100 F 0,078 kW
Capacity utilisation (including empty runs) 61 % Average power input 32-120 0,083 kW
Gross density of products transported 568 kg/m3 Average power input 40-40 F 0,045 kW
Wastage during distribution - % Average power input 40-60 F 0,085 kW
Installation into the building (A5) End of life (C1-C4)
Name ValueUnit Name Value Unit
Packaging waste for incineration (LDPE film) 0,02 kg Collected as mixed construction waste 5,7 kg
Packaging waste for incineration Transportation distance (C2) 100 km
0,41 kg
(Paper/Cardboard)
Aluminium for recycling 0,328 kg
An estimated RSL of 10 years can be used to facilitate building Steel for recycling (incl. cast iron) 2,95 kg
calculations. This is an EU consensus-based estimation, Copper for recycling (incl. brass) 0,199 kg
referenced in Appendix 7: Lot 11 – Circulators in Buildings,
Stainless steel for recycling 0,404 kg
prepared by AEA Energy & Environment for the European
Plastics for incineration (incl. rubber) 0,719 kg
Commission in the context of the Eco Design Directive.
Electronics for incineration w/energy 0,285 kg
Reference service life
Paper for incineration 0,214 kg
Name Value Unit
Landfilling 0,60 kg
Life Span according to the manufacturer 10 a
Reuse, recovery and/or recycling potentials (D), relevant
Operational energy use (B6)
scenario information
4 Environmental Product Declaration - Grundfos Holding A/S - MAGNA3 25,32-40/60/80/100/120, 32-40/60/80/100 F, 40-40/60 F (Cast iron)
Name Value Unit
A5, incineration w/energy recov. thermal energy 0,809 MJ
A5, incineration w/energy recov. electric energy 0,893 MJ
C3, steel for recycling (net amounts) 0,931 kg
C3, stainless steel for recycling (net amounts) 0,341 kg
C3, aluminium for recycling (net amounts) 0,004 kg
C3, copper for recycling (net amounts) 0,186 kg
C4, incineration w/energy recov. thermal energy 3,85 MJ
C4, incineration w/energy recov. electric energy 4,28 MJ
5 Environmental Product Declaration - Grundfos Holding A/S - MAGNA3 25,32-40/60/80/100/120, 32-40/60/80/100 F, 40-40/60 F (Cast iron)
LCA: Results
Characterization model: EN 15804 - 2012+A2 - 2019, PEF. By Decision no. 20170712-n of the IBU SVR, the modules B3, B4, B5 are
marked as MNR (module not relevant) as default. The LCA results in module B6 are given on a period of one year, according to PCR
Part B. To obtain the results from module B6 over the entire life cycle, the LCA results of module B6 must be multiplied by the
estimated RSL of 10 years. The indicator results for module B6 are declared for MAGNA3 25-40. B6 indicator results for other groups
can be derived by multiplying the B6 indicator results with the following factors:
MAGNA3 25-60: 1,68; MAGNA3 25-80: 2,32; MAGNA3 25-100: 3,06; MAGNA3 25-120: 3,7;
MAGNA3 32-40, 32-40 F: 1,36; MAGNA3 32-60, 32-60 F: 2,06; MAGNA3 32-80, 32-80 F: 2,72; MAGNA3 32-100, 32-100 F: 3,42;
MAGNA3 32-120: 3,64;
MAGNA3 40-40 F: 1,95; MAGNA3 40-60 F: 3,7
DESCRIPTION OF THE SYSTEM BOUNDARY (X = INCLUDED IN LCA; MND = MODULE OR INDICATOR NOT DECLARED; MNR
= MODULE NOT RELEVANT)
Benefits and
Construction loads beyond
Product stage Use stage End of life stage
process stage the system
boundaries
la ire ta m w a Ry lp p u s tro p s n a rT g n iru tc a fu n a M e h t m o rf tro p s n a rTe tis e h t o t e ta g y lb m e s s A e s U e c n a n e tn ia M ria p e R tn e m e c a lp e R tn e m h s ib ru fe R y g re n e la n o ita re p Oe s u re ta w la n o ita re p Oe s u n o itc u rts n o c -e Dn o itilo m e d tro p s n a rT g n is s e c o rp e ts a W la s o p s iD -e s u e R-y re v o c e R-g n ilc y c e Rla itn e to p
A1 A2 A3 A4 A5 B1 B2 B3 B4 B5 B6 B7 C1 C2 C3 C4 D
X X X X X X X MNR MNR MNR X X X X X X X
RESULTS OF THE LCA - ENVIRONMENTAL IMPACT according to EN 15804+A2: 1PCS of MAGNA3 pump
Parameter Unit A1-A3 A4 A5 B1 B2 B6 B7 C1 C2 C3 C4 D
GWP-total kg CO 2 eq 4.13E+01 7.85E-01 5.9E-01 0 0 3.72E+01 0 0 4.84E-02 1.12E-01 2.55E+00 -3.97E+00
GWP-fossil kg CO 2 eq 4.22E+01 7.89E-01 2.32E-02 0 0 3.69E+01 0 0 4.86E-02 1.11E-01 2.24E+00 -3.96E+00
GWP-
biogenic kg CO 2 eq -9.88E-01 -1.17E-02 5.67E-01 0 0 3.21E-01 0 0 -7.2E-04 9.62E-04 3.09E-01 -1.49E-03
GWP-luluc kg CO 2 eq 4.23E-02 7.33E-03 3.59E-05 0 0 4.01E-03 0 0 4.52E-04 1.2E-05 3.73E-05 -2.99E-03
kg CFC11
ODP 3.63E-08 1.03E-13 7.19E-14 0 0 6.81E-10 0 0 6.35E-15 2.04E-12 2.83E-13 -6.46E-12
eq
AP mol H+ eq 2.05E-01 5.09E-03 1.83E-04 0 0 7.88E-02 0 0 3.13E-04 2.36E-04 6.27E-04 -2.56E-02
EP-
kg P eq 5.67E-04 2.9E-06 3.52E-08 0 0 1.38E-04 0 0 1.78E-07 4.13E-07 2.99E-06 -3.99E-06
freshwater
EP-marine kg N eq 4.02E-02 2.49E-03 6.96E-05 0 0 1.89E-02 0 0 1.54E-04 5.66E-05 2.3E-04 -2.94E-03
EP-terrestrial mol N eq 3.37E-01 2.76E-02 8.54E-04 0 0 1.97E-01 0 0 1.7E-03 5.91E-04 2.96E-03 -3.14E-02
kg NMVOC
POCP 9.64E-02 4.81E-03 1.76E-04 0 0 5.03E-02 0 0 2.97E-04 1.51E-04 6.22E-04 -9.57E-03
eq
ADPE kg Sb eq 2.77E-03 5.25E-08 8.84E-10 0 0 5.71E-06 0 0 3.24E-09 1.71E-08 2.33E-09 -5.64E-04
ADPF MJ 5.78E+02 1.08E+01 2.32E-01 0 0 7.77E+02 0 0 6.65E-01 2.33E+00 1.04E+00 -4.35E+01
m3 world eq
WDP 1.45E+01 9.57E-03 7.26E-02 0 0 8.22E+00 0 0 5.9E-04 2.47E-02 2.55E-01 -5.68E-01
deprived
GWP = Global warming potential; ODP = Depletion potential of the stratospheric ozone layer; AP = Acidification potential of land and water; EP =
Eutrophication potential; POCP = Formation potential of tropospheric ozone photochemical oxidants; ADPE = Abiotic depletion potential for non-fossil
resources; ADPF = Abiotic depletion potential for fossil resources; WDP = Water (user) deprivation potential)
RESULTS OF THE LCA - INDICATORS TO DESCRIBE RESOURCE USE according to EN 15804+A2: 1PCS of MAGNA3 pump
Parameter Unit A1-A3 A4 A5 B1 B2 B6 B7 C1 C2 C3 C4 D
PERE MJ 1.3E+02 7.85E-01 6.2E+00 0 0 4.64E+02 0 0 4.84E-02 1.39E+00 3.56E+00 -6E+00
PERM MJ 9.52E+00 0 -6.15E+00 0 0 0 0 0 0 0 -3.38E+00 0
PERT MJ 1.4E+02 7.85E-01 4.79E-02 0 0 4.64E+02 0 0 4.84E-02 1.39E+00 1.82E-01 -6E+00
PENRE MJ 5.54E+02 1.08E+01 3.87E-01 0 0 7.77E+02 0 0 6.67E-01 2.33E+00 2.59E+01 -4.36E+01
PENRM MJ 2.5E+01 0 -1.55E-01 0 0 0 0 0 0 0 -2.49E+01 0
PENRT MJ 5.79E+02 1.08E+01 2.32E-01 0 0 7.77E+02 0 0 6.67E-01 2.33E+00 1.04E+00 -4.36E+01
SM kg 3.98E+00 0 0 0 0 0 0 0 0 0 0 0
RSF MJ 0 0 0 0 0 0 0 0 0 0 0 0
NRSF MJ 0 0 0 0 0 0 0 0 0 0 0 0
FW m3 4.43E-01 8.6E-04 1.71E-03 0 0 3.75E-01 0 0 5.3E-05 1.12E-03 6E-03 -1.37E-02
PERE = Use of renewable primary energy excluding renewable primary energy resources used as raw materials; PERM = Use of renewable primary
energy resources used as raw materials; PERT = Total use of renewable primary energy resources; PENRE = Use of non-renewable primary energy
excluding non-renewable primary energy resources used as raw materials; PENRM = Use of non-renewable primary energy resources used as raw
materials; PENRT = Total use of non-renewable primary energy resources; SM = Use of secondary material; RSF = Use of renewable secondary fuels;
NRSF = Use of non-renewable secondary fuels; FW = Use of net fresh water
6 Environmental Product Declaration - Grundfos Holding A/S - MAGNA3 25,32-40/60/80/100/120, 32-40/60/80/100 F, 40-40/60 F (Cast iron)
RESULTS OF THE LCA – WASTE CATEGORIES AND OUTPUT FLOWS according to EN 15804+A2:
1PCS of MAGNA3 pump
Parameter Unit A1-A3 A4 A5 B1 B2 B6 B7 C1 C2 C3 C4 D
HWD kg 2.96E-04 3.35E-11 5.96E-12 0 0 9.59E-08 0 0 2.07E-12 2.88E-10 5.87E-11 -2.13E-04
NHWD kg 1.51E+00 1.65E-03 1.83E-02 0 0 5.69E-01 0 0 1.02E-04 1.71E-03 6.84E-01 4E-01
RWD kg 1.45E-02 2.03E-05 9.85E-06 0 0 1.23E-01 0 0 1.25E-06 3.7E-04 3.53E-05 -1.49E-03
CRU kg 0 0 0 0 0 0 0 0 0 0 0 0
MFR kg 0 0 0 0 0 0 0 0 0 0 0 0
MER kg 0 0 0 0 0 0 0 0 0 3.88E+00 0 0
EEE MJ 0 0 8.93E-01 0 0 0 0 0 0 0 4.28E+00 0
EET MJ 5.51E-03 0 8.09E-01 0 0 0 0 0 0 0 3.85E+00 0
HWD = Hazardous waste disposed; NHWD = Non-hazardous waste disposed; RWD = Radioactive waste disposed; CRU = Components for re-use;
MFR = Materials for recycling; MER = Materials for energy recovery; EEE = Exported electrical energy; EET = Exported thermal energy
RESULTS OF THE LCA – additional impact categories according to EN 15804+A2-optional:
1PCS of MAGNA3 pump
Parameter Unit A1-A3 A4 A5 B1 B2 B6 B7 C1 C2 C3 C4 D
Disease
PM 2.68E-06 1.89E-08 9.63E-10 0 0 6.63E-07 0 0 1.16E-09 1.99E-09 4.37E-09 -3.94E-07
incidence
kBq U235
IR 1.83E+00 3.02E-03 1.56E-03 0 0 2.05E+01 0 0 1.86E-04 6.16E-02 5.51E-03 -2.53E-01
eq
ETP-fw CTUe 3.54E+02 7.73E+00 1.11E-01 0 0 2.16E+02 0 0 4.76E-01 7.28E-01 5.45E-01 -1.11E+01
HTP-c CTUh 3.78E-07 1.57E-10 5.52E-12 0 0 1.14E-08 0 0 9.67E-12 8.84E-11 4.6E-11 -4.98E-08
HTP-nc CTUh 5.08E-07 6.98E-09 1.49E-10 0 0 1.82E-07 0 0 4.3E-10 5.68E-09 2.7E-09 -2.01E-08
SQP SQP 2.17E+02 4.51E+00 7.35E-02 0 0 3.05E+02 0 0 2.78E-01 9.14E-01 2.07E-01 -1.04E+01
PM = Potential incidence of disease due to PM emissions; IR = Potential Human exposure efficiency relative to U235; ETP-fw = Potential comparative
Toxic Unit for ecosystems; HTP-c = Potential comparative Toxic Unit for humans (cancerogenic); HTP-nc = Potential comparative Toxic Unit for humans
(not cancerogenic); SQP = Potential soil quality index
Disclaimer 1 – for the indicator 'Potential Human exposure efficiency relative to U235'.
This impact category deals mainly with the eventual impact of low-dose ionizing radiation on human health of the nuclear fuel cycle. It
does not consider effects due to possible nuclear accidents, occupational exposure or radioactive waste disposal in underground
facilities. Potential ionizing radiation from the soil, radon and from some construction materials is also not measured by this indicator.
Disclaimer 2 – for the indicators 'abiotic depletion potential for non-fossil resources', 'abiotic depletion potential for fossil resources',
'water (user) deprivation potential, deprivation-weighted water consumption', 'potential comparative toxic unit for ecosystems', 'potential
comparative toxic unit for humans – cancerogenic', 'Potential comparative toxic unit for humans - not cancerogenic', 'potential soil
quality index'. The results of this environmental impact indicator shall be used with care as the uncertainties on these results are high
as there is limited experience with the indicator.
Disclaimer 3: JRC Technical Reports, Version 2, 2018 Page 6, for the indicator "EP-freshwater". This indicator has been calculated as
'kg P eq' as required in the characterization model EUTREND model, Struijs et al., 2009b, as implemented in ReCiPe;
References
EN 15804 Radio Equipment Directive
EN 15804:2012+A2:2019+AC:2021, Sustainability of DIRECTIVE 2014/53/EU OF THE EUROPEAN PARLIAMENT
construction works — Environmental Product Declarations — AND OF THE COUNCIL of 16 April 2014 on the harmonisation
Core rules for the product category of construction products. of the laws of the Member States relating to the making
available on the market of radio equipment
ISO 14025
Electromagnetic Compatibility (EMC) Directive
EN ISO 14025:2011, Environmental labels and declarations —
Type III environmental declarations — Principles and DIRECTIVE 2014/30/EU OF THE EUROPEAN PARLIAMENT
procedures. AND OF THE COUNCIL of 26 February 2014 on the
harmonistion of the laws of the Member States relating to
IBU 2021 electromagnetic compatibility
Institut Bauen und Umwelt e.V.: General Instructions for the Ecodesign Directive
EPD programme of Institut Bauen und Umwelt e.V., Version
2.0, Berlin: Institut Bauen und Umwelt e.V., 2021www.ibu- DIRECTIVE 2009/125/EC OF THE EUROPEAN PARLIAMENT
epd.com AND OF THE COUNCIL of 21 October 2009 establishing a
framework for the setting of
Standards ecodesign requirements for energy-related products
Machinery Directive EC 641/2009
DIRECTIVE 2006/42/EC OF THE EUROPEAN PARLIAMENT COMMISSION REGULATION (EC) No 641/2009 of 22 July
AND OF THE COUNCIL of 17 May 2006 on machinery 2009 implementing Directive 2005/32/EC of the European
Parliament and of the Council with regard to ecodesign
7 Environmental Product Declaration - Grundfos Holding A/S - MAGNA3 25,32-40/60/80/100/120, 32-40/60/80/100 F, 40-40/60 F (Cast iron)
requirements for glandless standalone circulators and EN 60335-2-51
glandless circulators integrated in products
EN 60335-2-51:2003-03 + A1:2008 + A2:2012, Household and
EC 622/2012 similar electrical appliances – Safety –Part 2-51: Particular
requirements for stationary circulation pumps for heating and
COMMISSION REGULATION (EU) No 622/2012 of 11 July service water installations
2012 amending Regulation (EC) No 641/2009 with regard to
ecodesign requirements for glandless standalone circulators EN 61000-3-2
and glandless circulators integrated in products
EN 61000-3-2:2014/2019, Electromagnetic compatibility (EMC)
DIRECTIVE 2011/65/EU – Part 3-2: Limits – Limits for harmonic current emissions
(equipment input current =16 A per phase)
DIRECTIVE 2011/65/EU OF THE EUROPEAN PARLIAMENT
AND OF THE COUNCIL of 8 June 2011 on the restriction of the EN 61000-3-3
use of certain hazardous
substances in electrical and electronic equipment EN 61000-3-3:2013-08/ A1:2019, Electromagnetic compatibility
(EMC) – Part 3-3:
DIRECTIVE 2015/863/EU Limits – Limitation of voltage changes, voltage fluctuations and
flicker in public low voltage supply systems, for equipment with
DIRECTIVE 2015/863/EU of 31 March 2015 amending Annex II rated current <= 16 A per phase and not subject to conditional
to Directive 2011/65/EU of the European Parliament and of the connection
Council as regards the list of restricted substances
EN 61000-6-2
ETSI EN 301 489-1
EN 61000-6-2:2008/2019, Electromagnetic compatibility (EMC)
ETSI EN 301 489-1 V2.2.0, Electromagnetic Compatibility – Part 6-2: Generic standards –Immunity for industrial
(EMC) standard for radio equipment and services; Part 1: environments
Common technical requirements
EN 16297-1
ETSI EN 301 489-17
EN 16297-1:2012-10, Pumps – Rotodynamic pumps –
ETSI EN 301 489-17 V3.2.0, Electromagnetic Compatibility Glandless circulators – Part 1:
(EMC) standard for radio equipment and services; Part 17: General requirements and procedures for testing and
Specific conditions for Broadband Data Transmission Systems calculation of energy efficiency index (EEI)
ETSI EN 300 328 V2.1.1 EN 16297-2
ETSI EN 300 328 V2.1.1, Wideband transmission systems; EN 16297-2:2012-10, Pumps – Rotodynamic pumps –
Data transmission equipment operating in the 2,4 GHz ISM Glandless circulators – Part 2: Calculation of energy efficiency
band and using wide band modulation techniques index (EEI) for standalone circulators
EN 809 EN 16297-3
EN 809:1998-10 + A1:2009, Pumps and pump units for liquids - EN 16297-3:2012, Pumps – Rotodynamic pumps –Glandless
Common safety requirements circulators – Part 3: Energy efficiency index (EEI) for circulators
integrated in products
EN 55014-1
ISO 14001
EN 55014-1:2017, Electromagnetic compatibility –
Requirements for household appliances, electric tools and EN ISO 14001:2015-09, Environmental management systems -
similar apparatus – Part 1: Emission Requirements with guidance for use
EN 55014-2 ISO 14025
EN 55014-2:2015, Electromagnetic compatibility – DIN EN /ISO 14025:2011-10, Environmental labels and
Requirements for household appliances, electric tools and declarations — Type III environmental declarations —
similar apparatus – Part 2: Immunity – Product family standard Principles and procedures
(CISPR 14-2:2015)
EN 15804
EN 50581:2012
EN 15804:2012-04+A1 2013, Sustainability of construction
EN 50581:2012, Technical documentation for the assessment works — Environmental Product Declarations — Core rules for
of electrical and electronic products with respect to the the product category of construction products
restriction of hazardous substances
PCR Part A
EN 60335-1
Institut Bauen und Umwelt e.V., Berlin (pub.): Product Category
EN 60335-1:2012/A11:2014/A13:2017, Household and similar Rules for Building-Related Products and Services, Product
electrical appliances – Safety – Part 1:General requirements Category Rules for Construction Products from the range of
Environmental Product Declarations of Institut Bauen und
8 Environmental Product Declaration - Grundfos Holding A/S - MAGNA3 25,32-40/60/80/100/120, 32-40/60/80/100 F, 40-40/60 F (Cast iron)
Umwelt (IBU), Part A: Calculation Rules for the Life Cycle
Assessment and Requirements on the Project Report, Version Candidate List of substances of very high concern (SVHCs) for
1.3. authorisation, European Chemicals Agency (ECHA), Helsinki,
Finland
PCR Part B
EUTREND model
Institut Bauen und Umwelt e.V., Berlin (pub.): Product Category Struijs et al., 2009b AEA Energy & Environment
Rules for Building-Related Products and Services, Product Circulators in Buildings
Category Rules for Construction Products from the range of
Environmental Product Declarations of Institut Bauen und Ecoinvent
Umwelt (IBU), Part B: Requirements on the EPD for Pumps for Ecoinvent v3.9.1
liquids and liquids with solids, Version 1.0 (2018)
LCA for Experts
Further references 10.7.1.28 Schema 8007
CPR
REACH Regulation (EC) No 1907/2006 of the European
REGULATION (EU) No 305/2011 OF THE EUROPEAN Parliament and of the Council of 18 December 2006 concerning
PARLIAMENT AND OF THE COUNCIL of 9 March 2011 laying the Registration, Evaluation, Authorisation and Restriction of
down harmonised conditions for the marketing of construction Chemicals (REACH) (Status: 27.06.2018)
products and repealing Council Directive 89/106/EEC
SVR
CML 2001
Advisory Board (formerly SVA)
Impact assessment characterization factors Institute of
Environmental Sciences, Leiden University, Netherlands Decision no.
20170712-n
ECHA candidate list
9 Environmental Product Declaration - Grundfos Holding A/S - MAGNA3 25,32-40/60/80/100/120, 32-40/60/80/100 F, 40-40/60 F (Cast iron)
Publisher
Institut Bauen und Umwelt e.V. +49 (0)30 3087748- 0
Hegelplatz 1 info@ibu-epd.com
10117 Berlin www.ibu-epd.com
Germany
Programme holder
Institut Bauen und Umwelt e.V. +49 (0)30 3087748- 0
Hegelplatz 1 info@ibu-epd.com
10117 Berlin www.ibu-epd.com
Germany
Author of the Life Cycle Assessment
Grundfos Holding A/S +45 87501400
Poul Due Jensens Vej 7 LCA_EPD@grundfos.com
8850 Bjerringbro www.grundfos.com
Denmark
Owner of the Declaration
Grundfos Holding A/S +45 87501400
Poul Due Jensens Vej 7 LCA_EPD@grundfos.com
8850 Bjerringbro www.grundfos.com
Denmark
10 Environmental Product Declaration - Grundfos Holding A/S - MAGNA3 25,32-40/60/80/100/120, 32-40/60/80/100 F, 40-40/60 F (Cast iron)
