ENVIRONMENTAL PRODUCT DECLARATION
as per ISO 14025 and EN 15804+A2
Owner of the Declaration Halbmond Teppichwerke GmbH
Publisher Institut Bauen und Umwelt e.V. (IBU)
Programme holder Institut Bauen und Umwelt e.V. (IBU)
Declaration number EPD-HBM-20230147-CBC1-EN
Issue date 05.05.2023
Valid to 04.05.2028
Tufted wall-to-wall carpet with PP backing and a pile material of PA
6 Econyl® with 100% recycled content
Halbmond Teppichwerke GmbH
www.ibu-epd.com | https://epd-online.com
General Information
Halbmond Teppichwerke GmbH Tufted wall-to-wall carpet with PP backing and a
pile material of PA 6 Econyl® with 100% recycled
content
Programme holder Owner of the declaration
IBU – Institut Bauen und Umwelt e.V. Halbmond Teppichwerke GmbH
Hegelplatz 1 Brückenstraße 1
10117 Berlin 08606 Oelsnitz
Germany Germany
Declaration number Declared product / declared unit
EPD-HBM-20230147-CBC1-EN tufted wall-to-wall carpet with PP backing and a pile material of PA 6 with
100% recycled content
This declaration is based on the product category rules: Scope:
Floor coverings, 01.08.2021 The manufacturer declaration applies to tufted wall-to-wall carpet with a PP
(PCR checked and approved by the SVR) backing, a pile material of PA 6 with 100% recycled content and a
maximum total pile weight of 1270 g/m2. The products are produced in
Oelsnitz/Vogtl., Germany.
Issue date LCA results for products with a maximum total pile weight of 745 g/m2 can
05.05.2023 be taken from the corresponding tables of the annexe. Specific data for
every product within the declared group of products in relation to its total
pile weight can be calculated by using equation 1 given in the annexe (see
Valid to annexe chapter: 'General Information on the annexe'). The declaration is
only valid in conjunction with a valid GUT-PRODIS license of the product.
04.05.2028 The owner of the declaration shall be liable for the underlying information
and evidence; the IBU shall not be liable with respect to manufacturer
information, life cycle assessment data and evidences.
The EPD was created according to the specifications of EN 15804+A2. In
the following, the standard will be simplified as EN 15804.
Verification
The standard EN 15804 serves as the core PCR
Independent verification of the declaration and data according to ISO
14025:2011
Dipl.-Ing. Hans Peters
internally X externally
(Chairman of Institut Bauen und Umwelt e.V.)
Florian Pronold Angela Schindler,
(Managing Director Institut Bauen und Umwelt e.V.) (Independent verifier)
Environmental Product Declaration - Halbmond Teppichwerke GmbH - Tufted wall-to-wall carpet with PP backing and a pile material of PA 6 Econyl® with 100% recycled
1 content
Product
characteristics according to EN 14041: 2018-05, Resilient,
Product description/Product definition textile and laminate floor coverings - Essential characteristics.
The declaration applies to tufted wall-to-wall carpet having a Additional product properties in accordance with EN 1307 can
surface pile of 100% recycled solution dyed polyamide 6 with a be found on the Product Information System PRODIS using the
maximum total pile weight of 1270 g/m2. The backing of the PRODIS registration number of the product (www.pro-dis.info)
carpet consists of a PP backing. The total recycled content of or on the manufacturer's technical information section.
the carpet is 54%. The chromojet printing system allows the
creation of various designs. For the placing on the market of Base materials/Ancillary materials
the specific product in the European Union/European Free Name Value Unit
Trade Association (EU/EFTA) (with the exception of Polyamide 6 55.3 %
Switzerland) Regulation (EU) No. 305/2011 Construction
Polyester 3.8 %
Product Regulation (CPR) applies. The product needs a
Polypropylene 2.6 %
Declaration of Performance (DoP) taking into consideration EN
14041:2018-05, Resilient, textile and laminate floor coverings - SBR Latex 14.0 %
Essential characteristics, and the CE-marking. The DoP of the Limestone 13.0 %
product can be found on the manufacturer's technical Aluminium Hydroxide 10.3 %
information section. For the application and use of the product
Additives 1.0 %
the respective national provisions apply.
The specific product covered by the EPD contains substances
Application listed in the ECHA candidate list (17.01.2023) or other
The use class of the specific product as defined in EN 1307 can carcinogenic, mutagenic or reprotoxic (CMR) substances in
be found in the Product Information System (PRODIS) using categories 1A or 1B which are not on the candidate list
the PRODIS registration number of the product. exceeding 0.1 percentage by mass: no The products are
registered in the GUT-PRODIS Information System. The
Technical Data PRODIS system ensures the compliance with limitations of
various chemicals and Volatile Organic Compound (VOC)-
Constructional data according to EN 1307 emissions and a ban on the use of all substances that are listed
as 'Substances of Very High Concern' (SVHC) under REACH.
Name Value Unit
Product Form Wall-to-wall carpet on rolls - Reference service life
Type of manufacture Tufted carpet - The service life of textile floor coverings strongly depends on
Yarn type PA 6 with 100% recycled content - the correct installation taking into account the declared use
classification and the adherence to cleaning and maintenance
Total carpet weight 2352 g/m2
instructions. A calculation of the reference service life according
Secondary backing PP backing - to ISO 15686 is not possible. Alternatively, a reference service
Total pile weight 1270 g/m2 life of 10 years can be assumed, during which the functional
and visual quality is guaranteed (BNB, Nutzungsdauer von
Performance data of the product in accordance with the
Bauteilen). The technical service life can be significantly longer.
declaration of performance with respect to its essential
LCA: Calculation rules
2 - municipal waste incineration
Declared Unit 3 - recovery in a cement plant
Name Value Unit A1-A3 Production:
Declared unit 1 m2 Energy supply and production of the basic material, processing
of secondary material, auxiliary material, transport of the
Grammage 2.352 kg/m2
material to the manufacturing site, emissions, waste water
The declared unit refers to 1 m2 produced textile floor covering. treatment, packaging material and waste processing up to the
The Output of module A5 'Assembly' is 1 m2 installed textile landfill disposal of residual waste (except radioactive waste).
floor covering. Benefits for generated electricity and steam due to the
The layer thickness of the specific product covered by the EPD incineration of production waste are aggregated. Biogenic
can be found on the Product Information System PRODIS using carbon that is stored in renewable material (packaging paper) is
the PRODIS registration number of the product (www.pro- taken into account as well as the associated carbon dioxide
dis.info) or on the manufacturer's technical information section. uptake from the air from which this biogenic carbon comes.
A4 Transport:
Transport of the packed textile floor covering from factory gate
System boundary to the place of installation.
Type of EPD:
Cradle-to-gate with options, module C1-C4, module D, and A5 Installation:
additional modules A4, A5, B1, B2. Installation of the textile floor covering, processing of
System boundaries of modules A, B, C, D: installation waste and packaging waste up to the landfill
Modules C3, C4 and D are indicated separately for three end- disposal of residual waste (except radioactive waste), the
of-life scenarios: production of the amount of carpet that occurs as installation
1 - landfill disposal waste including its transport to the place of installation.
Environmental Product Declaration - Halbmond Teppichwerke GmbH - Tufted wall-to-wall carpet with PP backing and a pile material of PA 6 Econyl® with 100% recycled
2 content
Generated electricity and steam due to the incineration of C3-1: Landfill disposal needs no waste processing.
waste are listed in the result table as exported energy. Biogenic C3-2: Impact from waste incineration (plant with R1>0.6),
carbon that is stored in renewable materials in packaging paper generated electricity and steam are listed in the result table as
is released as carbon dioxide emissions into the air at the end exported energy.
of life in module A5. Preparation of the floor and auxiliary C3-3: Collection of the carpet waste for recovery in the cement
materials (adhesives, fixing agents, PET connectors) are industry, waste processing (granulating), transport to the
beyond the system boundaries and not taken into account. cement plant, emissions from the incineration.
B1 Use: C4 Disposal
Indoor emissions during the use stage. After the first year, C4-1: Impact from landfill disposal,
noproduct-related Volatile Organic Compound (VOC) emissions C4-2: The carpet waste leaves the system in module C3-2,
are relevant due to known VOC decay curves of the product. C4-3: The pre-processed carpet waste leaves the system in
module C3-3.
B2 Maintenance:
Cleaning of the textile floor covering for a period of 1 year: D Recycling potential:
Vacuum cleaning – electricity supply Calculated benefits result from materials exclusive secondary
Wet cleaning – electricity, water consumption, production of the materials (net materials).
cleaning agent, waste water treatment. D-A5: Benefits for generated energy due to incineration of
The declared values in this module have to be multiplied by the packaging and installation waste (incineration plant with R1 >
assumed service life of the floor covering in the building in 0.6),
question. D-1: Benefits for generated energy due to landfill disposal of
carpet waste at the end-of-life,
B3 - B5: D-2: Benefits for generated energy due to incineration of carpet
The modules are not relevant within the assumed reference waste at the end-of-life (incineration plant with R1 > 0.6),
service life of 10 years. D-3: Benefits for saved fossil energy and saved inorganic
material due to recovery of the carpet in a cement plant.
B6 - B7:
No energy and water input are required for the operation of the Geographic Representativeness
carpet in the use stage. The modules do not cause any Land or region, in which the declared product system is
environmental impact. manufactured, used or handled at the end of the product´s
lifespan: Europe
C1 De-construction:
The floor covering is de-constructed manually and no additional
Comparability
environmental impact is caused.
Basically, a comparison or an evaluation of EPD data is only
possible if all the data sets to be compared were created
C2 Transport:
according to EN 15804 and the building context, respectively
Transport of the carpet waste to a landfill, to the municipal
the product-specific characteristics of performance, are taken
waste incineration plant (MWI) or to the waste collection facility
into account. Background data are taken from the GaBi
for recycling.
database, 2022-2. Remaining data gaps are covered by the
ecoinvent 3.7 database, 2020
C3 Waste processing:
LCA: Scenarios and additional technical information
Polyethylene packaging waste and installation waste are
Characteristic product properties of biogenic carbon considered to be incinerated in a municipal waste incineration
plant. Cardboard packaging waste is going to be recycled.
Name ValueUnit Preparation of the floor and auxiliaries (adhesives, fixing
Biogenic carbon content in accompanying kg agents, PET connectors etc.) are not taken into account.
0.013
packaging at factory gate C
Maintenance (B2)
1 kg biogenic Carbon is equivalent to 44/12 kg of CO
2
The values for cleaning refer to 1 m2 floor covering per year.
Depending on the application based on ISO 10874, the
technical service life recommended by the manufacturer and
the anticipated strain on the floor by customers, the case-
specific useful life can be established. Based on this useful life
Transport to the construction site (A4)
the effects of module B2 need to be calculated in order to
Name Value Unit obtain the overall environmental impacts.
Litres of fuel (truck, EURO 0-6 mix) 0.0055 l/100km Name Value Unit
Transport distance 700 km Maintenance cycle (vacuum cleaning) 208 Number /year
Capacity utilisation (including empty runs) 55 % Maintenance cycle (wet cleaning) 1,5 Number /year
Water consumption (wet cleaning) 0.004 m3
Cleaning agent (wet cleaning) 0.09 kg
Installation in the building (A5) Electricity consumption 0.314 kWh
Name Value Unit
For further information on cleaning and maintenance see
Material loss 0.212 kg www.halbmond.de
Environmental Product Declaration - Halbmond Teppichwerke GmbH - Tufted wall-to-wall carpet with PP backing and a pile material of PA 6 Econyl® with 100% recycled
3 content
If combinations of these scenarios have to be calculated this
should be done according to the following scheme:
Service life
EOL-impact = x % impact (Scenario 1)
Name Value Unit
+ y % impact (Scenario 2)
Life Span (according to BBSR) 10 a + z % impact (Scenario 3)
Corresponds to the with x % + y % + z % = 100 %
Declared product properties (at
specifications of EN -
the gate) and finishes
1307 Name ValueUnit
A wn h ea ns s inu sm tae ld le dq u ina l ait cy c o of r w dao nrk c, e C mo an nfo ur fm acs
t
uto
re
t rh 'se
-
C ano dll e 2c )ted as mixed construction waste (scenario 1 2.352 kg
with the manufacturer’s
instructions Collected separately waste type (scenario 3) 2.352 kg
instructions
Landfilling (scenario 1) 2.352 kg
Usage conditions, e.g. Use in areas defined by
Energy recovery (scenario 2) 2.352 kg
frequency of use, mechanical the use class according -
exposure to EN 1307 Energy recovery (scenario 3) 1.803 kg
Maintenance e.g. required According to the Recycling (scenario 3) 0.549 kg
frequency, type and quality and manufacturers - Reuse, recovery and/or recycling potentials (D), relevant
replacement of components instructions scenario information
Recovery or recycling potentials due to the three end-of-life
End of Life (C1-C4)
scenarios (module C) are indicated separately.
Three different end-of-life scenarios are declared and the
results are indicated separately in module C.
Recycling in the cement industry (scenario 3) The organic
Each scenario is calculated as a 100% scenario.
material of the carpet is used as an alternative fuel in a cement
Scenario 1: 100 % landfill disposal
kiln. It mainly substitutes for lignite (68.8 %), hard coal (23.6 %)
Scenario 2: 100 % municipal waste incineration (MWI)
and petrol coke (7.6 %). The inorganic material is substantially
with R1>0.6
integrated into the cement clinker and substitutes for original
Scenario 3: 100 % recovery in the cement industry
material input. VDZ e.V.
Environmental Product Declaration - Halbmond Teppichwerke GmbH - Tufted wall-to-wall carpet with PP backing and a pile material of PA 6 Econyl® with 100% recycled
4 content
LCA: Results
The LCA results refer to all declared products with a maximum total pile weight of 1270 g/m2. LCA results for products with a maximum
total pile weight of 745 g/m2 can be taken from the corresponding tables of the annexe. Results for specific products with any other
total pile weight can be calculated by using equation 1 given in the annexe (see annexe chapter: 'General Information on the annexe').
The declared result figures in module B2 have to be multiplied by the assumed service life (in years) of the floor covering in the building
under consideration. Information on non-relevant modules: Modules B3 - B7 are not relevant during the service life of the carpet.
Modules C1, C3/1, C4/2 and C4/3 cause no additional impact (see chapter "LCA: Calculation rules" in this document). All these
modules are declared and marked as 'modules not relevant/declared'. Module C2 represents the transport for scenarios 1, 2 and 3.
Column D represents module D/A5.
DESCRIPTION OF THE SYSTEM BOUNDARY (X = INCLUDED IN LCA; MND = MODULE OR INDICATOR NOT DECLARED; MNR
= MODULE NOT RELEVANT)
Benefits and
Construction loads beyond
Product stage Use stage End of life stage
process stage the system
boundaries
la ire ta m w a Ry lp p u s tro p s n a rT g n iru tc a fu n a M e h t m o rf tro p s n a rTe tis e h t o t e ta g y lb m e s s A e s U e c n a n e tn ia M ria p e R tn e m e c a lp e R tn e m h s ib ru fe R y g re n e la n o ita re p Oe s u re ta w la n o ita re p Oe s u n o itc u rts n o c -e Dn o itilo m e d tro p s n a rT g n is s e c o rp e ts a W la s o p s iD -e s u e R-y re v o c e R-g n ilc y c e Rla itn e to p
A1 A2 A3 A4 A5 B1 B2 B3 B4 B5 B6 B7 C1 C2 C3 C4 D
X X X X X X X MNR MNR MNR MND MND X X X X X
RESULTS OF THE LCA - ENVIRONMENTAL IMPACT according to EN 15804+A2: 1 m² floor covering
Parameter Unit A1-A3 A4 A5 B1 B2 C1 C2 C3/2 C3/3 C4/1 D D/1 D/2 D/3
GWP-total kg CO 2 eq 6.13E+00 1.42E-01 9.93E-01 0 4.16E-01 0 7.97E-03 3.97E+004.01E+00 1.67E-01 -3.46E-02 0 -2.69E-01 -1.46E-01
GWP-fossil kg CO 2 eq 6.12E+00 1.39E-01 9.44E-01 0 2.15E-01 0 7.83E-03 3.97E+004.01E+00 1.67E-01 -3.44E-02 0 -2.68E-01 -1.46E-01
GWP-
biogenic kg CO 2 eq 5.46E-03 1.8E-03 4.87E-02 0 4.16E-03 0 1.01E-04 4.89E-04 8.51E-04 -2.71E-08 -1.74E-04 0 -1.34E-03 -2.57E-04
GWP-luluc kg CO 2 eq 8.44E-03 7.88E-04 8.4E-04 0 1.96E-01 0 4.45E-05 6.65E-05 1.8E-04 8.11E-05 -3.72E-06 0 -2.87E-05 -7.9E-05
kg CFC11
ODP 2.27E-07 8.48E-15 2.05E-08 0 3.42E-08 0 4.78E-16 3.99E-13 5.76E-13 2.24E-13 -2.28E-13 0 -1.75E-12 -1.38E-13
eq
AP mol H+ eq 2.28E-02 8.43E-04 2.64E-03 0 8.32E-04 0 4.73E-05 5.63E-03 5.77E-03 4.94E-04 -4.47E-05 0 -3.46E-04 -6.5E-04
EP-
kg P eq 5.01E-04 4.23E-07 4.52E-05 0 5.19E-06 0 2.38E-08 3.07E-07 4.02E-07 3.11E-05 -4.64E-08 0 -3.57E-07 -1.75E-07
freshwater
EP-marine kg N eq 7.53E-03 4.13E-04 9.73E-04 0 1.97E-04 0 2.33E-05 2.85E-03 2.9E-03 1.09E-04 -1.22E-05 0 -9.46E-05 -1.86E-04
EP-terrestrial mol N eq 6.75E-02 4.59E-03 9.36E-03 0 2.83E-03 0 2.59E-04 3.16E-02 3.23E-02 1.2E-03 -1.31E-04 0 -1.01E-03 -2.03E-03
kg
POCP NMVOC 1.85E-02 7.81E-04 2.4E-03 4.18E-04 9.83E-04 0 4.4E-05 7.26E-03 7.39E-03 3.5E-04 -3.41E-05 0 -2.65E-04 -5.41E-04
eq
ADPE kg Sb eq 3.48E-05 1.18E-08 3.13E-06 0 2.3E-07 0 6.66E-10 1.55E-08 2.05E-08 1.16E-08 -5.13E-09 0 -3.95E-08 -1.49E-08
-4.54E -1.21E
ADPF MJ 1.01E+021.89E+009.42E+00 0 5.9E+00 0 1.06E-01 2.03E+002.52E+00 2.38E+00 -5.85E-01 0
+00 +01
m3 world
WDP eq 8.04E+00 1.27E-03 7.68E-01 0 9.99E-02 0 7.13E-05 4.67E-01 4.7E-01 -1.77E-03 -3.56E-03 0 -2.73E-02 -1.92E-02
deprived
GWP = Global warming potential; ODP = Depletion potential of the stratospheric ozone layer; AP = Acidification potential of land and water; EP =
Eutrophication potential; POCP = Formation potential of tropospheric ozone photochemical oxidants; ADPE = Abiotic depletion potential for non-fossil
resources; ADPF = Abiotic depletion potential for fossil resources; WDP = Water (user) deprivation potential)
RESULTS OF THE LCA - INDICATORS TO DESCRIBE RESOURCE USE according to EN 15804+A2: 1 m² floor covering
Parameter Unit A1-A3 A4 A5 B1 B2 C1 C2 C3/2 C3/3 C4/1 D D/1 D/2 D/3
PERE MJ 6.57E+01 1.08E-01 6.01E+00 0 3.68E+00 0 6.05E-03 2.95E-01 4.32E-01 1.95E-01 -1.58E-01 0 -1.21E+00 -2.43E-01
PERM MJ 5.9E-02 0 -5.9E-02 0 0 0 0 0 0 0 0 0 0 0
PERT MJ 6.57E+01 1.08E-01 5.95E+00 0 3.68E+00 0 6.05E-03 2.95E-01 4.32E-01 1.95E-01 -1.58E-01 0 -1.21E+00 -2.43E-01
PENRE MJ 8.82E+01 1.9E+00 9.73E+00 0 5.9E+00 0 1.07E-01 1.45E+01 1.5E+01 2.38E+00 -5.85E-01 0 -4.54E+00-1.21E+01
-1.25E -1.25E
PENRM MJ 1.28E+01 0 -3.01E-01 0 0 0 0 0 0 0 0 0
+01 +01
PENRT MJ 1.01E+02 1.9E+00 9.43E+00 0 5.9E+00 0 1.07E-01 2.03E+00 2.52E+00 2.38E+00 -5.85E-01 0 -4.54E+00-1.21E+01
SM kg 1.42E+00 0 1.28E-01 0 0 0 0 0 0 0 0 0 0 3.33E-01
RSF MJ 0 0 0 0 0 0 0 0 0 0 0 0 0 0
NRSF MJ 0 0 0 0 0 0 0 0 0 0 0 0 0 0
FW m3 1.9E-01 1.22E-04 1.82E-02 0 3.34E-03 0 6.84E-06 1.1E-02 1.12E-02 2.77E-05 -1.51E-04 0 -1.16E-03 -1.24E-03
PERE = Use of renewable primary energy excluding renewable primary energy resources used as raw materials; PERM = Use of renewable primary
energy resources used as raw materials; PERT = Total use of renewable primary energy resources; PENRE = Use of non-renewable primary energy
excluding non-renewable primary energy resources used as raw materials; PENRM = Use of non-renewable primary energy resources used as raw
materials; PENRT = Total use of non-renewable primary energy resources; SM = Use of secondary material; RSF = Use of renewable secondary fuels;
NRSF = Use of non-renewable secondary fuels; FW = Use of net fresh water
Environmental Product Declaration - Halbmond Teppichwerke GmbH - Tufted wall-to-wall carpet with PP backing and a pile material of PA 6 Econyl® with 100% recycled
5 content
RESULTS OF THE LCA – WASTE CATEGORIES AND OUTPUT FLOWS according to EN 15804+A2:
1 m² floor covering
Parameter Unit A1-A3 A4 A5 B1 B2 C1 C2 C3/2 C3/3 C4/1 D D/1 D/2 D/3
HWD kg 3.83E-03 9.08E-12 3.45E-04 0 4.19E-05 0 5.11E-13 3.28E-10 3.48E-10 3.65E-10 -7.98E-11 0 -6.23E-10 -1.71E-10
NHWD kg 6.81E-01 2.72E-04 9.06E-02 0 7.3E-03 0 1.53E-05 3.25E-01 3.25E-01 2.34E+00 -2.93E-04 0 -2.26E-03 -1.15E-01
RWD kg 1.76E-03 2.33E-06 1.64E-04 0 3.76E-04 0 1.31E-07 6.22E-05 9.74E-05 2.91E-05 -4.51E-05 0 -3.47E-04 -5.5E-05
CRU kg 0 0 0 0 0 0 0 0 0 0 0 0 0 0
MFR kg 0 0 3E-02 0 0 0 0 0 3.33E-01 0 0 0 0 0
MER kg 0 0 0 0 0 0 0 0 0 0 0 0 0 0
EEE MJ 0 0 6.88E-01 0 0 0 0 7.13E+00 0 0 0 0 0 0
EET MJ 0 0 1.24E+00 0 0 0 0 1.29E+01 5.31E+01 0 0 0 0 0
HWD = Hazardous waste disposed; NHWD = Non-hazardous waste disposed; RWD = Radioactive waste disposed; CRU = Components for re-use;
MFR = Materials for recycling; MER = Materials for energy recovery; EEE = Exported electrical energy; EET = Exported thermal energy
RESULTS OF THE LCA – additional impact categories according to EN 15804+A2-optional:
1 m² floor covering
Parameter Unit A1-A3 A4 A5 B1 B2 C1 C2 C3/2 C3/3 C4/1 D D/1 D/2 D/3
Disease
PM 1.62E-07 4.87E-09 1.66E-08 0 6.84E-08 0 2.74E-10 1.68E-08 1.77E-08 4.75E-09 -3.71E-10 0 -2.86E-09 -1.16E-08
incidence
kBq U235
IR 3.86E-01 3.42E-04 3.56E-02 0 6.78E-02 0 1.93E-05 9.47E-03 1.54E-02 4.29E-03 -7.64E-03 0 -5.87E-02 -7.27E-03
eq
ETP-fw CTUe 7.28E+011.31E+006.74E+00 0 2.69E+00 0 7.39E-02 7.43E-01 1.02E+002.32E+00 -1.26E-01 0 -9.68E-01 -2.4E+00
HTP-c CTUh 3.82E-09 2.65E-11 3.5E-10 0 6.21E-10 0 1.49E-12 4.42E-11 5.07E-11 1.04E-10 -5.87E-12 0 -4.55E-11 -4.24E-11
HTP-nc CTUh 1.43E-07 1.57E-09 1.33E-08 0 9.46E-09 0 8.85E-11 2.56E-09 2.88E-09 8.71E-09 -2.26E-10 0 -1.75E-09 -2.91E-09
SQP SQP ND ND ND ND ND ND ND ND ND ND ND ND ND ND
PM = Potential incidence of disease due to PM emissions; IR = Potential Human exposure efficiency relative to U235; ETP-fw = Potential comparative
Toxic Unit for ecosystems; HTP-c = Potential comparative Toxic Unit for humans (cancerogenic); HTP-nc = Potential comparative Toxic Unit for humans
(not cancerogenic); SQP = Potential soil quality index
No substantiated values can be given for the SQP indicator with the existing database.
The result figures given in module B2 refer to a period of 1 year because a reference service life is not declared. They have to be
multiplied by the assumed service life (in years) of the floor covering in the building under consideration.
Disclaimer 1 – for the indicator 'Potential Human exposure efficiency relative to U235'.
This impact category deals mainly with the eventual impact of low dose ionizingradiation on human health of the nuclear fuel cycle. It
does not consider effects due to possible nuclear accidents, occupational exposure nor due to radioactive waste disposal in
undergroundfacilities. Potential ionizing radiation from the soil, from radon and from some construction materials is also not measured
by this indicator.
Disclaimer 2 – for the indicators 'abiotic depletion potential for non-fossil resources', 'abiotic depletion potential for fossil resources',
'water (user) deprivation potential, deprivation-weighted water consumption', 'potential comparative toxic unit for ecosystems', 'potential
comparative toxic unit for humans – cancerogenic', 'Potential comparative toxic unit for humans - not cancerogenic', 'potential soil
quality index'.
The results of this environmental impact indicator shall be used with care as the uncertainties on these results are high or as there is
limited experienced with the indicator.
References
EN 1307 coverings – Environmental product declarations – Product
DIN EN 1307: 2014+A1:2016+A2:2018-05: Textile floor category rules
coverings - Classification
ISO 10874
EN 13501-1 DIN EN ISO 10874: 2012+A1:2021-04: Resilient, textile and
DIN EN 13501-1:2019-05: Fire classification of construction laminate floor coverings - Classification
products and building elements - Part 1: Classification using
data from reaction to fire tests ISO 14025
DIN EN /ISO 14025:2011-10/, Environmental labels and
EN 14041 declarations — Type III environmental declarations —
DIN EN 14041: 2018-05 and DIN EN 14041: 2008-05: Principles and procedures
Resilient, textile and laminate floor coverings - Essential
characteristics ISO 14040
DIN EN ISO 14040:2006+A1:2020 Environmental
EN 15804 management - Life cycle assessment - Principles and
DIN EN 15804:2012+A2:2019 + AC:2021, Sustainability of framework
construction works — Environmental Product Declarations —
Core rules for the product category of construction products ISO 14044
DIN EN ISO 14044:2006+A1:2018+A2:2020 Environmental
EN 16810 management - Life cycle assessment - Requirements and
DIN EN 16810: 2017-08: Resilient, textile and laminate floor guidelines
Environmental Product Declaration - Halbmond Teppichwerke GmbH - Tufted wall-to-wall carpet with PP backing and a pile material of PA 6 Econyl® with 100% recycled
6 content
September 2020
ISO 15686
ISO 15686: Buildings and constructed assets - Service life GaBi database
planning ISO 15686-1: 2011-05: Part 1: General principles and GaBi Software-System and Database for Life Cycle
framework ISO 15686-2: 2012-05: Part 2: Service life prediction Engineering, thinkstep AG, Leinfelden-Echterdingen, 2022-1
procedures ISO 15686-7: 2017-04: Part 7: Performance
evaluation for feedback of service life data from practice ISO PCR Part A
15686-8: 2008-06: Part 8: Reference service life and service- Product Category Rules for Building-Related Products and
life estimation Services Part A: Calculation Rules for the Life Cycle
Assessment and Requirements on the Project Report according
Regulation (EU) No. 305/2011 to EN 15804+A2:2019, V1.3, Berlin: Institut Bauen und Umwelt
Regulation No. 305/2011 Construction Products Regulation e.V. (IBU), August 2023
(CPR) of the European Council and of the European
Parliament, April 2011 PCR Part B
ProductCategory Rules for Building-Related Products and
General Instructions for the IBU-EPD Program Services Part B: Requirements on the EPD for floor coverings,
General Instructions for the EPD-Program of the Institut Bauen v1.0, Berlin: Institut Bauen und Umwelt e.V. (IBU), April 2023
und Umwelt e.V., The Preparation of Environmental Product
Declarations - EPDs, version 2.0, Institut Bauen und Umwelt PRODIS
e.V., Berlin, January 2021, www.ibu-epd.de Product Information System (PRODIS) of the European Carpet
Industry, Gemeinschaft umweltfreundlicher Teppichboden e.V
BNB, Nutzungsdauer von Bauteilen (GUT) and European Carpet and Rug Association (ECRA),
Bewertungssystem Nachhaltiges Bauen (BNB), Nutzungsdauer http://www.pro-dis.info
von Bauteilen, Bundesministerium des Inneren, für Bau und
Heimat, 24.02.2017 REACH
Regulation (EC) No 1907/2006 of the European Parliament and
ECHA candidate list of the Council of 18 December 2006 concerning the
Candidate List of substances of very high concern (SVHCs) for Registration, Evaluation, Authorisation and Restriction of
authorisation, 17.01.2023, European Chemicals Agency Chemicals (REACH), June 2017, last update: 17.01.2023
(ECHA), Helsinki, Finland
VDZ e.V.
ecoinvent Association of German Cement Works, Ed. Environ-mental
ecoinvent, Zurich, Switzerland, database version 3.7, published Data of the German Cement Industry 2020
Environmental Product Declaration - Halbmond Teppichwerke GmbH - Tufted wall-to-wall carpet with PP backing and a pile material of PA 6 Econyl® with 100% recycled
7 content
Publisher
Institut Bauen und Umwelt e.V. +49 (0)30 3087748- 0
Hegelplatz 1 info@ibu-epd.com
10117 Berlin www.ibu-epd.com
Germany
Programme holder
Institut Bauen und Umwelt e.V. +49 (0)30 3087748- 0
Hegelplatz 1 info@ibu-epd.com
10117 Berlin www.ibu-epd.com
Germany
Author of the Life Cycle Assessment
Gemeinschaft umweltfreundlicher Teppichboden +49 (0)241 96843 410
(GUT) e.V. mail@gut-ev.de
Schönebergstraße 2 www.gut-ev.org
52068 Aachen
Germany
Owner of the Declaration
Halbmond Teppichwerke GmbH +49 (0)37421 420
Brückenstraße 1 info@halbmond.de
08606 Oelsnitz www.halbmond.de
Germany
Environmental Product Declaration - Halbmond Teppichwerke GmbH - Tufted wall-to-wall carpet with PP backing and a pile material of PA 6 Econyl® with 100% recycled
8 content
