ENVIRONMENTAL PRODUCT DECLARATION
as per ISO 14025 and EN 15804+A2
Owner of the Declaration VELUX Group
Publisher Institut Bauen und Umwelt e.V. (IBU)
Programme holder Institut Bauen und Umwelt e.V. (IBU)
Declaration number EPD-VEL-20230505-CBA2-EN
Issue date 11.03.2024
Valid to 10.03.2029
VELUX frame extension LGI
VELUX A/S
www.ibu-epd.com | https://epd-online.com
General Information
VELUX A/S VELUX frame extension LGI
Programme holder Owner of the declaration
IBU – Institut Bauen und Umwelt e.V. VELUX Group
Hegelplatz 1 Ådalsvej 99
10117 Berlin 2970 Hørsholm
Germany Denmark
Declaration number Declared product / declared unit
EPD-VEL-20230505-CBA2-EN 1m² frame extension LGI.
The declared unit is based on the configuration of a standard size window
measuring 0.78 m x 1.178 m.
(The declared representative product of the product group comprise the
product with the highest mass.)
This declaration is based on the product category rules: Scope:
Windows and doors , 01.08.2021 Productline LGI - frame extension; manufactured by VELUX in Hungary for
(PCR checked and approved by the SVR) sale in Europe.
Declaration according to ISO 14025 and EN 15804 describing specific
Issue date environmental performance of the construction product.
The owner of the declaration shall be liable for the underlying information
11.03.2024
and evidence; the IBU shall not be liable with respect to manufacturer
information, life cycle assessment data and evidences.
Valid to
The EPD was created according to the specifications of EN 15804+A2. In
10.03.2029 the following, the standard will be simplified as EN 15804.
Verification
The standard EN 15804 serves as the core PCR
Independent verification of the declaration and data according to ISO
14025:2011
internally X externally
Dipl.-Ing. Hans Peters
(Chairman of Institut Bauen und Umwelt e.V.)
Florian Pronold Dr.-Ing. Nikolay Minkov,
(Managing Director Institut Bauen und Umwelt e.V.) (Independent verifier)
1 Environmental Product Declaration - VELUX A/S - VELUX frame extension LGI
Product
Performance data of the product with respect to its
Product description/Product definition characteristics in accordance with the relevant technical
The frame extension LGI consists of four pieces of frame made provision (no CE-marking).
of laminated pine wood to be fitted into the rebate of a VELUX
roof window, increasing the total frame height by 60 mm or Base materials/Ancillary materials
90mm. Name Value Unit
Wood painted/lacquered 97.8 %
To ensure a sufficient ventilation flow under the roofing material,
Steel 2.2 %
roof constructions are often provided with high counter battens.
The increased distance from the top of the battens to the REACH
insulation level leaves the roof window far away from the
insulation. To compensate for this, you can fit frame extension This product contains substances listed in the candidate list
LGI into the rebate of the roof window from the inside, (date: 09.08.2023) exceeding 0.1 percentage by mass: no.
increasing the total frame height and letting the window reach
the insulation.
Recycled content
Installation angle
Frame extensions can be installed regardless of roof pitch in all
roof constructions.
For the use and application of the product, the respective
national provisions at the place of use apply, in Germany for
example the building codes of the federal states and the The values stated in the table relate to the recycled material
corresponding national specifications. streams in VELUX production.
Application Reference service life
Frame extension for increasing the total frame height. The A calculation of the reference service life according to ISO
choice of roofing material is not affected by the use of a frame 15686 is not possible.
extension.
The Bundesinstitut für Bau, Stadt und Raumforschung/Federal
Technical Data office for building and regional planning (BBSR) table declares
The Declaration of Performance including relevant technical for the complete roof window a service life dependent on the
specifications and test methods/test standards can be applied window frame material between 25 and ≥ 50 years.
downloaded from the website www.velux.com/ce-marking. This includes extension frames as declared with this EPD.
Constructional data
Name Value Unit
Reaction to fire determination via window construction
Thermal resistancedetermination via window construction
Durability No performance determined
LCA: Calculation rules
Consideration of the production of raw materials (wood profile
Declared Unit and steel) and their processing (specific energy data: electrical
The declared unit is 1 m² related to a reference window, that energy from the national residual mix and thermal energy from
the frame extension is installed in connection with. natural gas, oil and biomass); transport of major materials to
The declared unit is based on the representative product the manufacturing site; assembly of semi-finished products to
measuring 0.78 m x 1.178 m. the final product; packaging material (including waste paper
The product LGIis manufactured in Hungary. input for paper and cardboard).
Declared unit and mass reference
End-of-Life stage C1, C2, C3:
Name Value Unit
C1: a manual demolition is assumed, resulting in indicator value
Declared unit 1 m2 "0".
Grammage 5.03 kg/m2 C2: For the transport to EoL by truck a distance of 50 km is
Layer thickness 0 m assumed.
C3: A scenario for the incineration of wood in a waste
Weight per area 4.63 kg/representative product
incineration plant (WIP) is assumed; metals are assumed to be
Weight per area 5.03 kg/declared unit
recycled.
The EoL-Scenario does not assume waste to be disposed of on
System boundary a landfill site. Module C4 is declared as"0".
Type of EPD: Cradle to gate - with options. The following life
cycle stages were considered: Benefits for the next product system D:
Resulting electrical and thermal energy from the WIP, avoiding
Production stage A1-A3: the generation of electricity and heat via fossil fuels, is
2 Environmental Product Declaration - VELUX A/S - VELUX frame extension LGI
considered. manufactured, used or handled at the end of the product´s
The amount of metals after the reduction due to the net-flow lifespan: Europe
calculations is sent to a recycling process. The effort for
recycling, as well as the benefit for the regained metals are
Comparability
declared in module D.
Basically, a comparison or an evaluation of EPD data is only
Contribution of waste flows is considered in the modules where possible if all the data sets to be compared were created
they occur. according to EN 15804 and the building context, respectively
the product-specific characteristics of performance, are taken
Geographic Representativeness into account. The software LCA FE 10.7 is used accompanied
Land or region, in which the declared product system is by the MLC database (version 2023.1, 2023).
LCA: Scenarios and additional technical information
Note: 1 kg of biogenic carbon is equivalent to 44/12 kg of CO .
2
Characteristic product properties of biogenic carbon
The following declared values refer to the declared unit of 1m².
Information on describing the biogenic carbon content at
factory gate
The declared biogenic content comprises the paper manual
and the packaging material consisting of cardboard, paper, PE,
EPS and steel. As module A5 is not declared, the information
on packaging supports further EoL calculations. Reference service life
Name ValueUnit Name Value Unit
kg Life Span (according to BBSR) 25 - 50 a
Biogenic carbon content in product 1.9
C
Biogenic carbon content in accompanying kg End of life (C1-C4)
0.5
packaging C Name Value Unit
The value refers to the following packaging material (per 1m²): Collected separately waste type 5.03 kg
Paper (manual): 0.001kg, Recycling 0.11 kg
Cardboard packaging: 1.175 kg, Energy recovery 4.92 kg
Paper insert: 0.012 kg,
PE-LD: 0.004 kg, Reuse, recovery and/or recycling potentials (D), relevant
EPS: 0.026 kg, scenario information
steel: 0.004 kg. Name Value Unit
Steel (net-flow-calculation) 0.13 kg/1m² product
Note: 1 kg of biogenic carbon is equivalent to 44/12 kg of CO .
2
3 Environmental Product Declaration - VELUX A/S - VELUX frame extension LGI
LCA: Results
The LCIA assessment is performed applying the characterisation factors "EN 15804+A2, EF 3.0".
DESCRIPTION OF THE SYSTEM BOUNDARY (X = INCLUDED IN LCA; MND = MODULE OR INDICATOR NOT DECLARED; MNR
= MODULE NOT RELEVANT)
Benefits and
Construction loads beyond
Product stage Use stage End of life stage
process stage the system
boundaries
la ire ta m w a Ry lp p u s tro p s n a rT g n iru tc a fu n a M e h t m o rf tro p s n a rTe tis e h t o t e ta g y lb m e s s A e s U e c n a n e tn ia M ria p e R tn e m e c a lp e R tn e m h s ib ru fe R y g re n e la n o ita re p Oe s u re ta w la n o ita re p Oe s u n o itc u rts n o c -e Dn o itilo m e d tro p s n a rT g n is s e c o rp e ts a W la s o p s iD -e s u e R-y re v o c e R-g n ilc y c e Rla itn e to p
A1 A2 A3 A4 A5 B1 B2 B3 B4 B5 B6 B7 C1 C2 C3 C4 D
X X X MND MND MND MND MNR MNR MNR MND MND X X X X X
RESULTS OF THE LCA - ENVIRONMENTAL IMPACT according to EN 15804+A2: 1 m² frame extension LGI
Parameter Unit A1-A3 C1 C2 C3 C4 D
Global Warming Potential total (GWP-total) kg CO 2 eq 1.8E+00 0 1.94E-02 9.88E+00 0 -3.16E+00
Global Warming Potential fossil fuels (GWP-fossil) kg CO 2 eq 8.86E+00 0 1.84E-02 2.97E+00 0 -3.15E+00
Global Warming Potential biogenic (GWP-biogenic) kg CO 2 eq -7.07E+00 0 8.06E-04 6.91E+00 0 -1.65E-02
Global Warming Potential luluc (GWP-luluc) kg CO 2 eq 1.79E-02 0 1.68E-04 7.12E-05 0 -1.93E-04
Depletion potential of the stratospheric ozone layer (ODP) kg CFC11 eq 9.65E-11 0 2.36E-15 1.17E-12 0 -2.28E-11
Acidification potential of land and water (AP) mol H+ eq 3.2E-02 0 3.64E-05 1.36E-03 0 -4.1E-03
Eutrophication potential aquatic freshwater (EP-freshwater) kg P eq 9.28E-05 0 6.62E-08 3.21E-07 0 -4.74E-06
Eutrophication potential aquatic marine (EP-marine) kg N eq 1.25E-02 0 1.5E-05 3.85E-04 0 -1.14E-03
Eutrophication potential terrestrial (EP-terrestrial) mol N eq 1.31E-01 0 1.71E-04 5.8E-03 0 -1.21E-02
Formation potential of tropospheric ozone photochemical oxidants kg NMVOC
3.37E-02 0 3.25E-05 1.07E-03 0 -3.29E-03
(POCP) eq
Abiotic depletion potential for non fossil resources (ADPE) kg Sb eq 3.35E-06 0 1.19E-09 1.07E-08 0 -7.63E-07
Abiotic depletion potential for fossil resources (ADPF) MJ 1.94E+02 0 2.47E-01 2.81E+00 0 -5.54E+01
m3 world eq
Water use (WDP) 1.79E+00 0 2.19E-04 9.46E-01 0 -3.17E-01
deprived
RESULTS OF THE LCA - INDICATORS TO DESCRIBE RESOURCE USE according to EN 15804+A2: 1 m² frame extension LGI
Parameter Unit A1-A3 C1 C2 C3 C4 D
Renewable primary energy as energy carrier (PERE) MJ 1.81E+02 0 1.79E-02 6.88E+01 0 -1.54E+01
Renewable primary energy resources as material utilization
MJ 7.02E+01 0 0 -6.81E+01 0 0
(PERM)
Total use of renewable primary energy resources (PERT) MJ 2.51E+02 0 1.79E-02 6.9E-01 0 -1.54E+01
Non renewable primary energy as energy carrier (PENRE) MJ 1.8E+02 0 2.48E-01 1.64E+01 0 -5.54E+01
Non renewable primary energy as material utilization (PENRM) MJ 1.48E+01 0 0 -1.36E+01 0 0
Total use of non renewable primary energy resources (PENRT) MJ 1.95E+02 0 2.48E-01 2.82E+00 0 -5.54E+01
Use of secondary material (SM) kg 1.07E+00 0 0 0 0 1.28E-01
Use of renewable secondary fuels (RSF) MJ 0 0 0 0 0 0
Use of non renewable secondary fuels (NRSF) MJ 0 0 0 0 0 0
Use of net fresh water (FW) m3 7.53E-02 0 1.97E-05 2.23E-02 0 -1.35E-02
RESULTS OF THE LCA – WASTE CATEGORIES AND OUTPUT FLOWS according to EN 15804+A2:
1 m² frame extension LGI
Parameter Unit A1-A3 C1 C2 C3 C4 D
Hazardous waste disposed (HWD) kg 3.85E-07 0 7.67E-13 4.49E-11 0 -2.84E-09
Non hazardous waste disposed (NHWD) kg 3.41E-01 0 3.77E-05 3.8E-01 0 4.59E-03
Radioactive waste disposed (RWD) kg 1.32E-02 0 4.63E-07 1.33E-04 0 -4.13E-03
Components for re-use (CRU) kg 0 0 0 0 0 0
Materials for recycling (MFR) kg 0 0 0 1.09E-01 0 0
Materials for energy recovery (MER) kg 0 0 0 0 0 0
Exported electrical energy (EEE) MJ 2.87E+00 0 0 1.37E+01 0 0
Exported thermal energy (EET) MJ 5.18E+00 0 0 2.47E+01 0 0
RESULTS OF THE LCA – additional impact categories according to EN 15804+A2-optional:
1 m² frame extension LGI
Parameter Unit A1-A3 C1 C2 C3 C4 D
Disease
Incidence of disease due to PM emissions (PM) 2.4E-06 0 2.35E-10 1.11E-08 0 -3.75E-08
incidence
Human exposure efficiency relative to U235 (IR) kBq U235 eq 1.1E+00 0 6.91E-05 2.02E-02 0 -6.82E-01
Comparative toxic unit for ecosystems (ETP-fw) CTUe 7.39E+01 0 1.75E-01 1.5E+00 0 -1.18E+01
Comparative toxic unit for humans (carcinogenic) (HTP-c) CTUh 3.12E-09 0 3.59E-12 1.09E-10 0 -6.82E-10
4 Environmental Product Declaration - VELUX A/S - VELUX frame extension LGI
Comparative toxic unit for humans (noncarcinogenic) (HTP-nc) CTUh 1.63E-07 0 2.02E-10 8.6E-09 0 -2.14E-08
Soil quality index (SQP) SQP 3.2E+03 0 1.03E-01 7.73E-01 0 -1.02E+01
Disclaimer 1 – for the indicator 'Potential Human exposure efficiency relative to U235'. This impact category deals mainly with the
eventual impact of low-dose ionizing radiation on human health of the nuclear fuel cycle. It does not consider effects due to possible
nuclear accidents, occupational exposure or radioactive waste disposal in underground facilities. Potential ionizing radiation from the
soil, radon and from some construction materials is also not measured by this indicator.
Disclaimer 2 – for the indicators 'abiotic depletion potential for non-fossil resources', 'abiotic depletion potential for fossil resources',
'water (user) deprivation potential, deprivation-weighted water consumption', 'potential comparative toxic unit for ecosystems', 'potential
comparative toxic unit for humans – cancerogenic', 'Potential comparative toxic unit for humans - not cancerogenic', 'potential soil
quality index'. The results of this environmental impact indicator shall be used with care as the uncertainties on these results are high
as there is limited experience with the indicator.
Disclaimer 3 – for 'potential soil quality index'. Due to a data lack in the foreground data of VELUX, the result has a very high
uncertainty and refers only to the background data, which contain respective information.
References
Standards EPD programme of Institut Bauen und Umwelt e.V., Version
2.0, Berlin: Institut Bauen und Umwelt e.V., 2021 www.ibu-
EN 15804 epd.com
EN 15804:2012+A2:2019+AC:2021, Sustainability of
construction works — Environmental Product Declarations — LCA FE 10.7 / MLC DB
Core rules for the product category of construction products. Sphera's LCA Software for Experts / Managed LCA Content
database, Sphera Solutions GmbH, Leinfelden-Echterdingen,
ISO 14025 database version 2023.1, 2023
EN ISO 14025:2011, Environmental labels and declarations —
Type III environmental declarations — Principles and PCR part A
procedures. Calculation Rules for the Life Cycle Assessment and
Requirements on the Project Report according to EN
ISO 15686 15804+A2:2019, version 1.3, IBU, 2022
ISO 15686-1:2011-05: Buildings and constructed assets -
Service life planning PCR part B
Requirements on the EPD for Windows and doors, version
Further References 01.08.2021, IBU
BBSR REACH/candidate list
BBSR, 24.02.2017, Nutzungsdauer von Bauteilen nach BNB Regulation (EC) No 1907/2006: Registration, Evaluation,
Authorisation and Restriction of Chemicals (REACH)
IBU 2021
Institut Bauen und Umwelt e.V.: General Instructions for the
5 Environmental Product Declaration - VELUX A/S - VELUX frame extension LGI
Publisher
Institut Bauen und Umwelt e.V. +49 (0)30 3087748- 0
Hegelplatz 1 info@ibu-epd.com
10117 Berlin www.ibu-epd.com
Germany
Programme holder
Institut Bauen und Umwelt e.V. +49 (0)30 3087748- 0
Hegelplatz 1 info@ibu-epd.com
10117 Berlin www.ibu-epd.com
Germany
Author of the Life Cycle Assessment
Angela Schindler Umweltberatung 07553 919 9456
Tüfinger Str. 12 angela@schindler-umwelt.de
88682 Salem www.schindler-umwelt.de
Germany
Daxner & Merl GmbH +43 676 849477826
Schleifmühlgasse 13/24 office@daxner-merl.com
1040 Wien www.daxner-merl.com
Austria
Owner of the Declaration
VELUX Group +4545164726
Ådalsvej 99 jakob.roerbech@velux.com
2970 Hørsholm www.velux.com
Denmark
6 Environmental Product Declaration - VELUX A/S - VELUX frame extension LGI
