ENVIRONMENTAL PRODUCT DECLARATION
as per ISO 14025 and EN 15804+A2
Owner of the Declaration VELUX Group
Publisher Institut Bauen und Umwelt e.V. (IBU)
Programme holder Institut Bauen und Umwelt e.V. (IBU)
Declaration number EPD-VEL-20230188-IBB1-EN
Issue date 10.08.2023
Valid to 09.08.2028
VELUX Interior roller blinds
VELUX A/S
www.ibu-epd.com | https://epd-online.com
1. General Information
VELUX A/S VELUX Interior roller blinds
Programme holder Owner of the declaration
IBU – Institut Bauen und Umwelt e.V. VELUX Group
Hegelplatz 1 Ådalsvej 99
10117 Berlin 2970 Hørsholm
Germany Denmark
Declaration number Declared product / declared unit
EPD-VEL-20230188-IBB1-EN 1 m² of VELUX interior roller blinds
This declaration is based on the product category rules: Scope:
Sun protection systems, 01.08.2021 100 % of the production volume of the current collection of VELUX interior
(PCR checked and approved by the SVR) roller blinds produced at the production sites in Denmark (Gåsdal
Bygningsindustri A/S), France (Velsol France) and the Czech Republic
(BKR ČR, s.r.o.), covering the variants DKL and RFL
Issue date The owner of the declaration shall be liable for the underlying information
and evidence; the IBU shall not be liable with respect to manufacturer
10.08.2023
information, life cycle assessment data and evidences.
The EPD was created according to the specifications of EN 15804+A2. In
Valid to
the following, the standard will be simplified as EN 15804.
09.08.2028
Verification
The standard EN 15804 serves as the core PCR
Independent verification of the declaration and data according to ISO
14025:2011
internally X externally
Dipl.-Ing. Hans Peters
(Chairman of Institut Bauen und Umwelt e.V.)
Florian Pronold Dr. Matthew Fishwick,
(Managing Director Institut Bauen und Umwelt e.V.) (Independent verifier)
1 Environmental Product Declaration - VELUX A/S - VELUX Interior roller blinds
2. Product
categories 1A or 1B which are not on the candidate list,
2.1 Product description/Product definition exceeding 0.1 percentage by mass:
Manually operated blackout roller blinds (DKL) and translucent
• not investigated with suppliers
roller blinds (RFL) are made for installation in VELUX roof
3) 'Biocide products were added to this construction product or
windows. VELUX interior blinds are available in a wide range of
it has been treated with biocide products (this then concerns a
colours and designs. In both blinds, the cloth is made of coated
treated product as defined by the (EU) Regulation on Biocidal
polyester. The control bar, top fascia and side rails are made of
Products No. 528/2012):
anodised or white-painted aluminium.
The two blinds are of the size 1178 mm x 780 mm = 0.929 m2 • no
For the placing on the market of the product in the European
2.6 Manufacture
Union/European Free Trade Association (EU/EFTA) (with the
Extruded aluminium profiles that are either anodised or coated,
exception of Switzerland) Regulation (EU) No. 305/2011 (CPR)
are bought from external suppliers. Depending on the size of
applies. The product needs a declaration of performance taking
the interior roller blinds, they are either bought cut-to-length or
into consideration EN 1873:2005, Prefabricated accessories for
as profiles to be cut before assembly. The other parts are also
roofing - Individual rooflights of plastics - Product specification
bought from other internal suppliers or external suppliers. The
and test methods and the CE-marking. For the application and
main production process then consists in assembling the final
use the respective national provisions apply.
product and its packaging before shipment.
2.2 Application
The blinds are made for installation in VELUX roof windows. The factories are ISO 9001 certified.
The VELUX blackout roller blind offers blackout for darkness
2.7 Environment and health during manufacturing
anytime. Ideal for bedrooms to ensure a good night's sleep or a
All factories are ISO 14001 and ISO 45001 certified.
daytime nap. VELUX translucent roller blind provides basic
privacy whilst still allowing in natural light. Perfect for living
2.8 Product processing/Installation
rooms, offices and playrooms. The blinds can be combined with
Interior roller blinds are for installation in VELUX roof windows.
exterior sun screening products, electric or solar window
It is easily clicked onto the top brackets pre-fitted on the
operators and interior insect screens.
window, leaving both hands free during the remaining part of
2.3 Technical Data the installation.
The declared values in the table relate to the reference product
2.9 Packaging
DKL (dark variant) in combination with VELUX roof window with
The packaging usually consists of:
2-layer insulating glass unit (--70, Uw = 1.3 [W/(m2K)]). For
- cardboard
other covered product combination specific values please
- paper insert
contact epd.support@velux.com.
Name Value Unit The use of other packaging materials is possible, but
U-value reduction ΔU 0.27 W/(m²K) insignificant in terms of quantity.
Improved insulation 20 % Cardboard and paper are usually recycled.
Solar energy transmittance (gtot) 0.38 -
2.10 Condition of use
Improved g-value 17 %
The material composition of VELUX interior roller blinds does
Shading factor (Fc-value) 0.83 - not change over their service life.
Performance data of the product in accordance with the
2.11 Environment and health during use
declaration of performance with respect to its essential
VELUX interior roller blinds do not contain any pollutants that
characteristics according to
could be released during use.
• EN 1873:2005, Prefabricated accessories for roofing -
Individual rooflights of plastics - Product specification Environmental protection: According to current knowledge,
and test methods hazards to water, air and soil cannot arise when the products
are used as intended.
2.4 Delivery status
The product is available in pre-defined sizes covering 0.55 m x
Health protection: According to current knowledge, no health
0.7 m to 1.34 m x 1.6 m.
hazards or impairments are to be expected.
2.5 Base materials/Ancillary materials
2.12 Reference service life
Composition of the VELUC interior roller blind DKL (size 1178
It is not possible to calculate the reference service life
mm x 780 mm = 0.929 m2): according to ISO 15686. The service life based on a
Aluminium 0.972 kg manufacturer's testing is 10 years. The corresponding
Steel 0.073 kg utilization scenario is declared in Chapter 4.
Polyester cloth 0.150 kg
other plastic parts 0.102 kg 2.13 Extraordinary effects
Fire
1) 'This product/article/at least one partial article contains Not classified for fire performance.
substances listed in the candidate list (date: 02.03.2022) Water
exceeding 0.1 percentage by mass: In the event of unforeseen exposure to water (flood), no
• no adverse effects on human health or the environment are to be
2) 'This product/article/at least one partial article contains other expected.
carcinogenic, mutagenic, reprotoxic (CMR) substances in
2 Environmental Product Declaration - VELUX A/S - VELUX Interior roller blinds
Mechanical destruction of the materials or the carbon content of the plastic parts,
In the event of unforeseen mechanical destruction, VELUX recycling or energy recovery is preferable and common.
interior roller blinds must be replaced; no adverse effects on
human health or the environment are to be expected. Waste code according to the European Waste List (Regulation
on the European Waste List):
2.14 Re-use phase 17 02 03 plastics
VELUX interior roller blinds can be dismantled manually without 17 04 14 mixed metals
any problems. The metal parts are usually recycled, and the
plastic parts are sent for thermal recycling for energy recovery. 2.16 Further information
Further documentation on the products, technical data sheets,
2.15 Disposal BIM files, etc. can be found at:
VELUX interior roller blinds are mostly inert and can be www.velux.com
disposed of in an appropriate landfill. However, due to the value
3. LCA: Calculation rules
fractions reach the end-of-waste state after having been sorted
3.1 Declared Unit and transported to a recycler. The combustible material
The declared unit for interior roller blinds is 1 m². (plastics) is assumed to be thermally treated in a municipal
Declared unit waste incineration plant.
Name Value Unit
Module D includes the benefits and burdens associated with
Declared unit 1 m2 recycling metals beyond the system boundary, resulting from
Grammage 1.4 kg/m2 the treatment of recycled materials from the point of end-of-
waste to the point of substitution (as loads) and substitution of
In addition to the declared product DKL, the lighter version RFL
primary resources (as benefits).
(related to the amount of aluminium and cloth) is included in the
It also includes the benefits and burdens associated with
EPD, hence following a conservative approach for the version
energy recovery from plastic waste in a municipal waste
RFL.
incineration plant, as modelled in Module C3.
3.2 System boundary In Module D, only net flows of metals leaving the product
system are considered.
Type of EPD: Cradle to gate with options, with modules C1 –
C4, and module D (A1-A3, C1-C3, D and additional modules).
3.3 Estimates and assumptions
No further assumptions and estimates relevant to the result had
The production of VELUX interior roller blinds (modules A1-
to be made beyond the points made in this chapter 3 and in
A3) includes raw material extraction, energy generation, waste
chapter 4.
treatment and all transports up to the factory gate. In
accordance with COUNCIL REGULATION (EU) No 333/2011, 3.4 Cut-off criteria
secondary metals are modeled as part of the product system
No data available from the company survey was neglected.
from the moment they are available as unmixed scrap.
These include, among other things, material use, energy
Waste or secondary fuels are not used for production.
demand (heat, electricity), packaging materials of raw materials
(insofar as they are generated as waste) and product
Module A4 is not declared due to large variances in transport
packaging, consumables in production, waste treatment and
distances between the production site and the construction site,
the transport of all inputs and outputs.
where the product is installed.
With this approach, mass and energy flows below 1 % were
also accounted for. No processes were neglected that would
Module A5: The products are delivered to the construction site
have been known to the project managers and would have
ready to be installed. Manual installation is assumed; electricity
contributed significantly to the indicators of the impact
consumption related to electric drilling machines, screw drivers,
assessment.
etc. is considered to be negligible. Paper and cardboard are
recycled; it is assumed that these fractions reach the end-of- 3.5 Background data
waste state after having been sorted and transported to a Ecoinvent v3.8 (2021, cut-off) is used as the background
recycler (as a conservative choice). No packaging waste is database.
landfilled.
3.6 Data quality
Modules B1 to B7 are not relevant for the product under The foreground data are based on extensive and detailed data
consideration or no significant environmental impacts occur. collection at the production site. The foreground data could be
fully linked with corresponding data records from the
Module C1 includes manual dismantling, with no significant background database Ecoinvent v3.8 (2021, cut-off).
environmental impact. The background data was updated in 2021. Thus, the quality of
the foreground and background data can be rated as very
Module C2 comprises the transport of the dismantled VELUX good.
interior roller blind to a sorting plant and then to a waste
incineration plant for the thermally treated plastic fraction. 3.7 Period under review
The LCA data represents the production conditions for the year
Modules C3/C4: given the complexity of the inventoried 2021.
products, a mixed end-of-life scenario is modelled, allowing the
3.8 Geographic Representativeness
different materials to follow their most likely path. As a rule of
thumb, metals are recycled and plastics are incinerated (also Land or region, in which the declared product system is
due to the very limited data availability on plastics recycling and manufactured, used or handled at the end of the product´s
its benefits). Metals are recycled; it is assumed that these lifespan: Europe
3 Environmental Product Declaration - VELUX A/S - VELUX Interior roller blinds
3.9 Allocation Allocation of reuse, recycling and recovery was avoided by the
No co-products are generated during the production of the cut-off approach in the foreground model in line with DIN EN
VELUX products. Sorted production scrap of the different 15804.
metals, notably aluminium, is considered a secondary material
with no economic value (so no burdens allocated) and 3.10 Comparability
considered in the quantification of net flows leaving the product Basically, a comparison or an evaluation of EPD data is only
system. This approach is chosen to ensure a coherent possible if all the data sets to be compared were created
quantification of net flows entering module D. according to EN 15804 and the building context, respectively
the product-specific characteristics of performance, are taken
No processes were modelled as part of the foreground model into account.
that would have required an allocation of multi-input processes. Ecoinvent v3.8 (2021, cut-off) has been used as the
Background datasets on municipal waste incineration plants background database.
were taken from ecoinvent without any modification.
4. LCA: Scenarios and additional technical information
Name Value Unit
Characteristic product properties of biogenic carbon
Reference service life
Information on describing the biogenic carbon content at according to manufacturer's 10 a
factory gate declaration
Name ValueUnit Reference service life - a
kg Declared product properties The product has passed
Biogenic carbon content in product - -
C (at the gate) and finishes internal quality controls
Biogenic carbon content in accompanying kg Design application
n.a.
packaging C parameters (if instructed by
Installation according to
the manufacturer), including
assembly instructions and -
the references to the
state of the art.
appropriate practices and
Module A5
application codes
The products are delivered to the construction site ready to be
installed. Manual installation is assumed; electricity An assumed quality of Carried out in accordance
consumption related to electric drilling machines, screwdrivers, work, when installed in with the manufacturer's -
etc. is considered to be negligible. accordance with the instructions.
Paper and cardboard are recycled; it is assumed that these manufacturer’s instructions
fractions reach the end-of-waste state after having been sorted Outdoor environment, (for
and transported to a recycler over 150 km with a lorry of 16-32 outdoor applications), e.g.
metric tons, EURO6 (as a conservative choice). weathering, pollutants, UV
Not applicable -
No packaging waste is landfilled. and wind exposure, building
The use of multi-way pallets is not taken into account as orientation, shading,
packaging material. temperature
Indoor environment (for
The declared products are
Reference service life indoor applications), e.g.
intended for installation -
temperature, moisture,
inside a building.
chemical exposure
Usage conditions, e.g. Standard use in any type of
frequency of use, building, i.e. opening/closing -
mechanical exposure 2 times a day
The declared products are
Maintenance e.g. required designed for a reference life
frequency, type and quality of 10 years. They are
-
and replacement of maintained by cleaning water
components at the discretion of the
building occupants.
Module B1
The products are assumed to have no direct emissions during
the use phase. The indicator values of Module B1 are thus 0.
For biogenic carbon storage, see the table above.
Module B2
For interior roller blinds, no impacts related to maintenance are
inventoried in module B2. Annual cleaning is neglected.
Module B6
Interior roller blinds do not consume operational energy.
Module C1
Manual de-installation is assumed, electricity consumption
4 Environmental Product Declaration - VELUX A/S - VELUX Interior roller blinds
related to electric screw drivers, etc. is considered to be The net amounts of the metals leaving the product system are
negligible. Thus, no environmental impacts are declared in considered as 'use of secondary material' in Module D.
module C1.
Module C4
Module C2 As stated above, it is assumed that 100 % of the plastic parts
Given the complexity of the inventoried products, a mixed end- are treated in a waste incineration plant with an efficiency R1
of-life scenario is modelled, allowing the different materials to < 0.6 (according to the ecoinvent dataset used); 25.57 % of the
follow their most likely path. It should also be noted that the lower heating value of the plastic parts are recovered as heat
deconstruction and waste treatment scenario can vary a lot, and 13.0 % as electricity. Recovered energy is reported as
depending on the actual situation. Thus, a generic end-of-life 'exported energy' and considered in Module D.
scenario is assumed. As a rule of thumb, metals are recycled,
plastics are incinerated (also due to the very limited availability Module D
of information on plastics recycling and its benefits). Module D contains the benefits and loads beyond the system
The combustible material (mainly plastics) is assumed to be boundary related to the recycling of metals, which result from
transported 50 km with a lorry of 16-32 metric tons, EURO6 to the treatment of recycled materials from the point of end-of-
an incineration plant. waste status to the point of substitution (as loads) and the
Metals are recycled; it is assumed that these fractions reach the substitution of primary resources (as benefits).
end-of-waste state after having been sorted and transported to It also includes the benefits and loads related to the energy
a recycler over 150 km with a lorry of 16-32 metric tons, recovery from plastic wastes in a municipal waste incineration
EURO6. plant (MWIP) as modelled in Modules A3, A5 and C3. Due to a
lack of data for plastics from de-construction activities, the
Module C3 substitution potential of recycled plastics is not taken into
A consumption of 0.03 kWh/kg of electricity for shredding and account.
sorting and 0.437 MJ/kg of diesel fuel for internal logistics are Only net flows leaving the product system are considered in
taken into account to disassemble the product. The recovered module D.
material leaves the product system as 'materials for recycling'.
5 Environmental Product Declaration - VELUX A/S - VELUX Interior roller blinds
5. LCA: Results
DESCRIPTION OF THE SYSTEM BOUNDARY (X = INCLUDED IN LCA; ND = MODULE OR INDICATOR NOT DECLARED; MNR =
MODULE NOT RELEVANT)
Benefits and
Construction loads beyond
Product stage Use stage End of life stage
process stage the system
boundaries
la ire ta m w a Ry lp p u s tro p s n a rT g n iru tc a fu n a M e h t m o rf tro p s n a rTe tis e h t o t e ta g y lb m e s s A e s U e c n a n e tn ia M ria p e R tn e m e c a lp e R tn e m h s ib ru fe R y g re n e la n o ita re p Oe s u re ta w la n o ita re p Oe s u n o itc u rts n o c -e Dn o itilo m e d tro p s n a rT g n is s e c o rp e ts a W la s o p s iD -e s u e R-y re v o c e R-g n ilc y c e Rla itn e to p
A1 A2 A3 A4 A5 B1 B2 B3 B4 B5 B6 B7 C1 C2 C3 C4 D
X X X MND X MND MND MNR MNR MNR MND MND X X X X X
RESULTS OF THE LCA - ENVIRONMENTAL IMPACT according to EN 15804+A2: 1 m² VELUX interior roller blind DKL
Parameter Unit A1-A3 A5 C1 C2 C3 C4 D
GWP-total kg CO 2 eq 2.01E+01 6.62E-01 0 2.4E-02 4.87E-02 5.98E-01 -1.43E+01
GWP-fossil kg CO 2 eq 2.06E+01 1.83E-01 0 2.4E-02 2.89E-02 5.98E-01 -1.42E+01
GWP-biogenic kg CO 2 eq -4.99E-01 4.79E-01 0 0 1.98E-02 0 0
GWP-luluc kg CO 2 eq 5.12E-02 5.88E-06 0 9.77E-06 3.21E-05 1.04E-05 -5.23E-02
ODP kg CFC11 eq 2.25E-06 3.3E-09 0 5.63E-09 1.78E-09 3.57E-09 -4.8E-07
AP mol H+ eq 1.3E-01 9.57E-05 0 1.36E-04 1.1E-04 1.44E-04 -9.09E-02
EP-freshwater kg P eq 8.24E-04 1.15E-07 0 1.77E-07 3.74E-06 3.27E-07 -5.35E-04
EP-marine kg N eq 2.14E-02 3.63E-05 0 4.89E-05 3.53E-05 6.05E-05 -1.35E-02
EP-terrestrial mol N eq 2.29E-01 4.03E-04 0 5.39E-04 4.01E-04 6.57E-04 -1.49E-01
kg NMVOC
POCP 6.71E-02 1.13E-04 0 1.54E-04 1.07E-04 1.67E-04 -4.4E-02
eq
ADPE kg Sb eq 1.11E-04 4.89E-08 0 8.04E-08 5.03E-08 8.64E-08 1.23E-04
ADPF MJ 2.32E+02 2.16E-01 0 3.7E-01 3.99E-01 1.12E-01 -1.29E+02
m3 world eq
WDP 4.25E+00 9.57E-04 0 1.21E-03 9.92E-04 6.8E-03 -1.9E+00
deprived
GWP = Global warming potential; ODP = Depletion potential of the stratospheric ozone layer; AP = Acidification potential of land and water; EP =
Eutrophication potential; POCP = Formation potential of tropospheric ozone photochemical oxidants; ADPE = Abiotic depletion potential for non-fossil
resources; ADPF = Abiotic depletion potential for fossil resources; WDP = Water (user) deprivation potential)
RESULTS OF THE LCA - INDICATORS TO DESCRIBE RESOURCE USE according to EN 15804+A2: 1 m² VELUX interior roller
blind DKL
Parameter Unit A1-A3 A5 C1 C2 C3 C4 D
PERE MJ 2.42E+01 5.51E+00 0 5.22E-03 5.04E-02 9.49E-03 -1.72E+01
PERM MJ 5.76E+00 -5.51E+00 0 0 -2.55E-01 0 0
PERT MJ 3E+01 3.37E-03 0 5.22E-03 -2.04E-01 9.49E-03 -1.72E+01
PENRE MJ 2.22E+02 2.64E+00 0 3.7E-01 3.18E-07 7.44E+00 -1.3E+02
PENRM MJ 9.93E+00 -2.6E+00 0 0 0 -7.33E+00 0
PENRT MJ 2.32E+02 2.16E-01 0 3.7E-01 3.18E-07 1.13E-01 -1.3E+02
SM kg 1.47E-01 0 0 0 0 0 1.12E+00
RSF MJ 0 0 0 0 0 0 0
NRSF MJ 0 0 0 0 0 0 0
FW m3 1.64E-01 5.21E-05 0 4.03E-05 9.52E-05 3.01E-04 -9.35E-02
PERE = Use of renewable primary energy excluding renewable primary energy resources used as raw materials; PERM = Use of renewable primary
energy resources used as raw materials; PERT = Total use of renewable primary energy resources; PENRE = Use of non-renewable primary energy
excluding non-renewable primary energy resources used as raw materials; PENRM = Use of non-renewable primary energy resources used as raw
materials; PENRT = Total use of non-renewable primary energy resources; SM = Use of secondary material; RSF = Use of renewable secondary fuels;
NRSF = Use of non-renewable secondary fuels; FW = Use of net fresh water
RESULTS OF THE LCA – WASTE CATEGORIES AND OUTPUT FLOWS according to EN 15804+A2:
1 m² VELUX interior roller blind DKL
Parameter Unit A1-A3 A5 C1 C2 C3 C4 D
HWD kg 3.22E-03 5.77E-07 0 9.42E-07 3.18E-07 4.55E-07 1.85E-03
NHWD kg 5.08E+00 1.59E-02 0 2.48E-02 1.62E-03 2E-02 -3.43E+00
RWD kg 1.09E-03 3.05E-06 0 5.34E-06 3.6E-06 7.31E-07 -4.02E-04
CRU kg 0 0 0 0 0 0 0
MFR kg 1.46E-01 3.25E-01 0 0 3.25E-01 0 0
MER kg 0 0 0 0 0 0 0
EEE MJ 2.72E-02 3.38E-01 0 0 0 3.38E-01 0
EET MJ 5.36E-02 6.66E-01 0 0 0 6.66E-01 0
6 Environmental Product Declaration - VELUX A/S - VELUX Interior roller blinds
HWD = Hazardous waste disposed; NHWD = Non-hazardous waste disposed; RWD = Radioactive waste disposed; CRU = Components for re-use;
MFR = Materials for recycling; MER = Materials for energy recovery; EEE = Exported electrical energy; EET = Exported thermal energy
RESULTS OF THE LCA – additional impact categories according to EN 15804+A2-optional:
1 m² VELUX interior roller blind DKL
Parameter Unit A1-A3 A5 C1 C2 C3 C4 D
Disease
PM 1.51E-06 1.65E-09 0 2.65E-09 1.74E-09 9.72E-10 -1.18E-06
incidence
IR kBq U235 eq 5.56E-01 9.25E-04 0 1.6E-03 1.38E-03 3.87E-04 -1.5E-01
ETP-fw CTUe 5.04E+02 2.05E-01 0 2.93E-01 2.35E-01 1.49E+00 -2.88E+02
HTP-c CTUh 3E-08 2.71E-11 0 1.17E-11 6.34E-12 1.21E-10 -1.58E-08
HTP-nc CTUh 4.82E-07 3.45E-10 0 3.37E-10 2.06E-10 1.05E-09 -2.45E-07
SQP SQP 7.16E+01 1.81E-01 0 3.15E-01 5.39E-02 3.77E-02 -1.87E+01
PM = Potential incidence of disease due to PM emissions; IR = Potential Human exposure efficiency relative to U235; ETP-fw = Potential comparative
Toxic Unit for ecosystems; HTP-c = Potential comparative Toxic Unit for humans (cancerogenic); HTP-nc = Potential comparative Toxic Unit for humans
(not cancerogenic); SQP = Potential soil quality index
Disclaimer 1 – for the indicator “Potential Human exposure efficiency relative to U235”. This impact category deals mainly with the
eventual impact of low-dose ionizing radiation on human health of the nuclear fuel cycle. It does not consider effects due to possible
nuclear accidents, occupational exposure or radioactive waste disposal in underground facilities. Potential ionizing radiation from the
soil, radon and from some construction materials is also not measured by this indicator.
Disclaimer 2 – for the indicators “abiotic depletion potential for non-fossil resources”, “abiotic depletion potential for fossil resources”,
“water (user) deprivation potential, deprivation-weighted water consumption”, “potential comparative toxic unit for ecosystems”,
“potential comparative toxic unit for humans – cancerogenic”, “Potential comparative toxic unit for humans - not cancerogenic”,
“potential soil quality index”. The results of this environmental impact indicator shall be used with care as the uncertainties on these
results are high as there is limited experience with the indicator.
6. LCA: Interpretation
Figure 1 illustrates the relative contributions of the different of the impacts over the product life cycle (modules A1-C4) and
modules along the life cycle of thecdeclared products. mainly related to the recycling potential of aluminium.
The use of renewable primary energy is mainly caused by the
share of renewable energy in the electricity mix, thus the
production stage is the main driver of this impact category; the
same holds also for the use of non-renewable primary energy.
Material use of primary energy is negligible and related to
plastic parts of the product and packaging material. The
material use of primary energy is transferred to its energy use
when the materials containing primary energy are incinerated
with energy recovery.
Non-hazardous waste as the quantitatively most relevant waste
flows is mainly caused in upstream processes (mining and
Figure 1: Relative environmental impacts of the different processing of aluminium); hazardous and radioactive waste are
life cycle stages for the VELUX interior roller blind DKL mainly caused by the European electricity mix used during the
(Modules A1-C4 = 100%) use phase.
The largest part of environmental impacts is caused during In addition to the declared product DKL, the lighter version RFL
production (modules A1-A3) of the interior roller blind. The (related to the amount of aluminium and cloth) is included in the
contributions of the other modules of the product life cycle are EPD. LCAs for these versions have not been calculated
not significant. specifically. Hence, no statement can be made on the variance
regarding these products.
Benefits and burdens beyond the system boundary (module D)
are in the order of 20 % to 60% (with the exception of the ODP)
7. Requisite evidence
7.1 Formaldehyde Not applicable; not tested based on applicable product
Not tested based on applicable product standard. standard.
7.2 MDI 7.4. Fire gas toxicity
Not tested based on applicable product standard. Not tested based on applicable product standard.
7.3 Checking of pre-treatment of substances used 7.5 VOC emissions
according to AltholzVO Not tested based on applicable product standard.
8. References
7 Environmental Product Declaration - VELUX A/S - VELUX Interior roller blinds
IBU programme documents Requirements with guidance for use.
IBU (2021) ECHA-List
IBU (2021): General Instructions for the EPD Programme of the The Candidate List of substances of very high concern,
Institut Bauen & Umwelt e.V. (General Instructions for the IBU available via https://echa.europa.eu/nl/-/four-newsubstances-
EPD Programme). Version 2.0, Institut Bauen & Umwelt, Berlin. added-to-the-candidate-list.
IBU (2017) Regulation on biocidal products
IBU (2007): PCR Teil A: PCR Part A: Calculation rules for the REGULATION (EU) No 528/2012 OF THE EUROPEAN
life cycle assessment and requirements for the project report. PARLIAMENT AND OF THE COUNCIL of 22 May 2012
Version 1.8., Institut Bauen & Umwelt, Berlin. concerning the making available on the market and use of
biocidal products.
IBU (2023)
IBU (2023): PCR Part B: Requirements on the EPD for sun Regulation (EU) Nr. 305/2011(CPR)
protection systems. Version 2023/04, Institut Bauen & Umwelt, REGULATION (EU) No 305/2011 OF THE EUROPEAN
Berlin. PARLIAMENT AND OF THE COUNCIL of 9 March 2011 laying
down harmonised conditions for the marketing of construction
Standards and legal documents products and repealing Council Directive 89/106/EEC.
EN 15804 COUNCIL REGULATION (EU) No 333/2011
EN 15804:2012+A2:2019 + AC:2021, Sustainability of COUNCIL REGULATION (EU) No 333/2011 of 31 March 2011
construction works - Environmental product declarations - Core establishing criteria determining when certain types of scrap
rules for the product category construction products. metal cease to be waste under Directive 2008/98/EC of the
European Parliament and of the Council.
ISO 14025
DIN EN ISO 14025:2006-07, Environmental labels and European Waste List (Waste index)
declarations - Type III Environmental declarations - Principles http://www.gesetze-im-internet.de/avv/anlage.htm
and procedures.
Additional references
ISO 14044
DIN EN ISO 14044:2006-07, Environmental management - Life Weidema et al. (2013)
cycle assessment - Requirements and guidance (ISO Weidema, B., C. Bauer, R. Hischier, C. Mutel, T. Nemecek, J.
14044:2006); German and English versions EN ISO Reinhard, C.O. Vadenbo, G. Wernet (2013): Overview and
14044:2006. methodology, Data quality guideline for the ecoinvent database
version 3. ecoinvent report no. 1
ISO 9001 (v3), St. Gallen, Schweiz.
DIN EN ISO 9001:2015, Quality management systems -
Requirements. ecoinvent 3.8
ecoinvent 3.8, LCA database, 12/2021. Ecoinvent centre,
ISO 14001 Zürich.
DIN EN ISO 14001:2015: Environmental management The literature referred to in the Environmental Product
systems - Requirements with guidance for use. Declaration must be listed in full.Standards already fully quoted
in the EPD do not need to be listed here again.
ISO 45001 The current version of PCR Part A and PCR Part B of the PCR
ISO 45001:2018-03, Occupational health and safety document on which they are based must be referenced.
management systems -
8 Environmental Product Declaration - VELUX A/S - VELUX Interior roller blinds
Publisher
Institut Bauen und Umwelt e.V. +49 (0)30 3087748- 0
Hegelplatz 1 info@ibu-epd.com
10117 Berlin www.ibu-epd.com
Germany
Programme holder
Institut Bauen und Umwelt e.V. +49 (0)30 3087748- 0
Hegelplatz 1 info@ibu-epd.com
10117 Berlin www.ibu-epd.com
Germany
Author of the Life Cycle Assessment
Dr. Frank Werner - Umwelt & Entwicklung + 41 (0)44 241 39 06
Kammelenbergstrasse 30 frank@frankwerner.ch
9011 St. Gallen http://www.frankwerner.ch/
Switzerland
Owner of the Declaration
VELUX Group +4545164726
Ådalsvej 99 jakob.roerbech@velux.com
2970 Hørsholm www.velux.com
Denmark
9 Environmental Product Declaration - VELUX A/S - VELUX Interior roller blinds
