Environmental Product
Declaration
In accordance with ISO 14025 and EN 15804 +A2
Owner of the declaration: PRODUCT NAME:
Superwood A/S
Exterior cladding of
Program holder and publisher:
Superwood, Fully
The Norwegian EPD foundation impregnated, surface
treated twice
Declaration number:
NEPD-3705-2649-EN
Registration unmber:
NEPD-3705-2649-EN
MANUFACTURER:
Issue date: 14.09.2022 Superwood A/S
Valid to: 14.09.2027
The Norwegian
EPD Foundation
General information
Product: Owner of the declaration:
Exterior cladding of Superwood, Fully impregnated, Superwood A/S
surface treated twice Contact person: Sofie Mora Kristensen
Phone: +45 7687 3200
Program Operator: e-mail: smk@superwood.dk
The Norwegian EPD Foundation
Post Box 5250 Majorstuen, 0303 Oslo, Norway Manufacturer:
Tlf: +47 23 08 80 00 Superwood A/S, Palsgaardvej 3, DK-7362 Hampen,
e-mail: post@epd-norge.no Denmark
Declaration Number: Place of production:
NEPD-3705-2649-EN Hampen, Denmark
This declaration is based on Product Management system:
Category Rules: FSC (SA-COC-007725) valid 11.09.20-10.09.25,
NPCR Part A:2021 Construction products and PEFC (SA-PEFC/COC-007725) valid 11.09.20-10.09.25
services Ver 2
NPCR 015 Part B for wood and wood-based products Organisation no:
4.0 26434602
Statements: Issue date:
The owner of the declaration shall be liable for the 14.09.2022
underlying information and evidence. EPD Norway
shall not be liable with respect to manufacturer, life
Valid to:
cycle assessment data and evidences.
14.09.2027
Declared unit:
Year of study:
1 m2 produced exterior cladding of Superwood, fully
Consumption data: 2021. LCA spring 2022.
impregnated, surface treated twice
Comparability:
Functional unit:
EPD of construction products may not be
1 m2 exterior cladding of Superwood, fully
comparable if they do not comply with EN 15804:A2
impregnated, surface treated twice, cradle to grave,
and seen in a building context.
reference service life 60 years
Verification: The EPD has been worked out by:
Independent verification of the declaration and Oddbjørn Dahlstrøm Andvik
data, according to ISO14025:2010 Asplan Viak AS
Internal ☐ External ☒
Independent verifier approved by EPD Norway Approved (Manager of EPD Norway)
EPD for the best environmental decision 2
Product
Product description:
Impregnated, planed wood from FSC and PEFC certified spruce (Picea abies), from Norway, Sweden
and Finland, for outdoor use above the ground. The wood is impregnated without the use of heavy
metals and organic solvents. The impregnation protects the tree completely into the core so that the
tree is protected against rot and fungus. The process takes place without the use of water, so the
wood is dry and can be used immediately after impregnation. The surface treatment is applied
mechanically and in a protected environment at the factory. Manufacturer for surface treatment is
Teknos, Teknoclade 3371.
Product specification:
Main application area is outdoor cladding (in all known cladding profiles), but noise barriers,
windscreens, railings, roofing tables and more are other natural applications. The cladding boards
can be delivered with and without surface treatment from the factory. This EPD yields for
impregnated cladding with two coats of surcace treatment.
The EPD encompasses all dimensions and profiles of the exterior of Superwood, with painted surface
(full cover). Painted surface (full cover) is 2 coats of paint from the factory (180 g paint m2).
Materials kg/m2 %
Woody of spruce, dry weight 7,77 83,0 %
Water, in wood, 18% 1,40 15,0 %
Impregnating, SC200 0,0079 0,084 %
Surafce treatment (paint) 0,180 1,92%
Total, without surface treatment 9,36 100 %
Packaging, plastic 0,02 kg / m2 0,02
Technical data:
Superwood has a density of 436,8 kg / m3, with moisture content of 16-20% (18% standard).
Superwood is protected from rotting, fungus and blue mold according to DS / EN 335, user class 3:
above ground contact. For Declaration of Performance (DoP), FSC certificate and complementary
information, see www.superwood.dk.
Standard dimension is 21 mm * 145 mm. Thickness of 21 mm is used in calculations. For 1 m2 of
covering cladding, 6,90 running meters of Superwood (dimensjon 0,145 m) is consumed.
Market:
The EPD includes transport to and sales in Denmark, Norway, Sweden and Germany.
Reference service life, product:
Reference service life is 60 years according to PCR. The actual service life depends on climatic
conditions and external impacts, such as construction and maintenance.
Reference service life, building:
Reference service life is 60 years according to PCR. The actual service life depends on climatic
conditions and external impacts.
EPD for the best environmental decision 3
Declared unit:
1 m2 produced exterior cladding of Superwood, fully impregnated, surface treated twice.
Data quality:
Production data is based on consumption data from 2021. Wood is splitted, impregnated and
profiled in Denmark. For sawn wood A1-A3 LCA impacts (GWP fossil and resource use) are based on
EPD of Finnish sawn and planed timber (RTS_124_21), EPD of Stora Enso Classic Sawn (S-P-02150)
and EPD Moelven (NEPD-2546-1284-NO). For surface treatment A1-A3 LCA impacts (GWP fossil and
resource use) are based on EPD for water-borne exterior paints from Teknos (RTS_13_18. Remaining
data is based on Ecoinvent v3.8, allocation, cut-off by classification (Nov 2021) and SimaPro v
9.3.0.3. Characterization factors have been used from EN15804:2012 + A2: 2019. Ecoinvent
processes are adjusted to improve representativeness (change of electricity mix).
Allocation:
Allocation has been made according to EN15804:2012 + A2: 2019. For sawn wood, economic
allocation has been used. For the production of Superwood, all consumption and waste are mass-
allocated for the production of impregnated wood. Primary production of recycled materials is
allocated to the main product where the material was used.
System boundary:
Flow sheet for manufacturing (A1-A3) and transport (A4) of Superwood is shown below.
EPD for the best environmental decision 4
N
A
o
1 : S a w n
w o o drd
ic s p ru c e
T ra
An 2s :
p o rt
MECdo a te r ia ls / E n e r g y :le
c tric ity , h e a t fro m w o o d c h ipO
2 g a s , im p re g n a tio n (S C 2 0 0ie
s e l fo r in te rn a l tra n s p o rt, lig hil,
p a c k a g in g
A 3 :S u p e rw o o d
D e n m a r k :S
p littin g , im p re g n a tio n ,
p ro file s a w in g
W a s te
s ,
),
t fu e l
AS 1u -Ap 3 : 1 me
r w o o
2d Ac 4 : T rao
n s tru
nc s ptio on rt to
s ite
LCA: Calculation rules
Cut-off criteria:
All major raw materials and all the essential energy is included. The production process for raw
materials and energy flows that are included with very small amounts (<1%) are not included. This
cut-off rule does not apply for hazardous materials or substances.
Calculation of biogenic carbon content:
Sequestration and emissions of biogenic carbon is calculated according to NS-EN 16485: 2014. This
approach is based on the modularity principle of EN 15804: emissions should be counted in the
module in which it actually occurs. The calculation of biogenic carbon content and conversion to
carbon dioxide is done according to the NS-EN 16449: 2014. The contribution to GWP from biogenic
carbon is shown for each module under core environmental impact indicators GWP-biogenic.
370 kg / m3 dry weight for Superwood has a carbon content converted to carbon dioxide of 678,6 kg
CO per m3 wood or 14,25 kg CO per m2 wood (21 mm thickness). The wood is from sustainable
2 2
forestry and is FSC and PEFC certified.
LCA: Scenarios and additional technical information
The following information describe the scenarios in the different modules of the EPD. All numbers
are pr m2 Superwood.
Transport from production place to assembly/user (A4)
All production normally takes place directly from Hampen to construction site or via retail. It is
considered a scenario of 200 km on a truck> 32 t. The A4 distance is calculated as average distance
for the Danish market. Additional distances estimated for other markets are given in the table
below.
Capacity utilisation (incl. Type of Fuel/Energy value
Type Distance KM
return) % vehicle consumption (l/t)
Lorry, >32t,
Truck 53% 200 0,017 l/tkm 3,4 l/t
EURO 6
Type Distance truck Distance boat A4, GWP fossil, kg CO2-eq/m2
Denmark 200 0 0,132
Norway (Oslo) 340 160 0,238
Sweeden (Örebro) 590 160 0,402
Germany (Berlin) 500 0 0,329
Assembly (A5)
It is assumed 5% spill at installation and 0,021 MJ/m2 energy consumption (1 MJ/m3) at construction
site. Waste treatment of the packaging is included in A5.
Unit Value
Auxiliary (paint) Kg 0
Water consumption m3 0
Electricity consumption kWh 0,00583
Other energy carriers MJ 0
Material loss Kg 5%: 0,459
Plastic packaging Kg 0,02
Dust in the air kg 0
Use (B1)
This stage includes no activities or emissions related to the product.
Maintenance (B2)/Repair (B3)
For painted surface (surcafe treated twice) a new coat of paint 1-6 months after installation and
every 7 years (total of 9 coats) is assumed during the building reference service life (B2). The
frequency of maintenance can be different and should always be considered in relation to the
EPD for the best environmental decision 5
intended use, construction and climatic conditions. Before each surface treatment, the surface is
cleaned with detergent and water.
10% replacement of cladding for repair (B3) is assumed during the building reference service life.
Unit Value
Maintenance cycle year 7
Paint kg 0,81
Detergent kg 0,018
Water consumption litre 0,378
Electricity consumption MJ 0
Other energy carriers MJ 0
Material loss Kg 10%: 0,917
Replacement (B4)/Refurbishment (B5)
Reference service life is 60 years according to PCR. The actual service life depends on climatic
conditions and external impacts, such as construction and maintenance. B4 and B5 includes no
activities or impacts related to the product.
Operational energy (B6) and water consumption (B7)
When used as an external cladding, the product has no operational energy or water use.
End of Life (C1, C3, C4)
The product is without heavy metals. The waste processing is assumed as wood waste treated with
incineration with energy recovery.
Unit Value
Hazardous waste disposed Kg 0
Collected as mixed construction waste Kg 9,18
Reuse Kg 0
Recycling Kg 0
Energy recovery Kg 9,18
To landfill Kg 0
Transport to waste processing (C2)
Type Capacity utilisation (incl. return) % Type of vehicle Distance km Fuel consumption Value (l/t)
Truck 36,67 % (Ecoinvent) Lorry 16-32t, Euro 5 50 0,045 l/tkm 2,3 l/t
The average distance for transport of wood waste is assumed to be 50 km.
Benefits and loads beyond the system boundaries (D)
The benefits of exported energy from energy recovery in a treatment facility is calculated with
substitution of Norwegian electricity market mix and Norwegian district heating mix (SSB 2020).
Conversion factors for efficiencies and losses from waste to delivered energy are included.
Unit Value
Substitution of electrical energy MJ 4,18
Substitution of thermal energy MJ 129,0
Substitution of raw materials kg 0
EPD for the best environmental decision 6
For the manufacturing process (A3 Superwood) 100% renewable electricity from Danish wind power is used in calculations (Guarantee of Origin
certificates). LCA results (GWP) calculated without the use of Guarantee of Origin is provided under Additional Norwegian requirements.
System boundaries (X=included, MND= module not declared, MNR=module not relevant)
Benefits & loads
Product stage Assembly stage Use stage End of life stage beyond system
boundary
EPD for the best environmental decision 7
slairetam
waR
tropsnarT
gnirutcafunaM
tropsnarT ylbmessA
esU
ecnanetniaM
riapeR
tnemecalpeR tnemhsibrufeR
esu
ygrene
lanoitarepO
esu
retaw
lanoitarepO
noitilomed
noitcurtsnoc-eD
tropsnarT
gnissecorp
etsaW
lasopsiD
-gnilcyceR-yrevoceR-esueR
laitnetop
LCA: Results
A1 A2 A3 A4 A5 B1 B2 B3 B4 B5 B6 B7 C1 C2 C3 C4 D
X X X X X X X X X X X X X X X X X
Core environmental impact indicators
Indicator Unit A1-A3 A4 A5 B2 B3 C1 C2 C3 C4 D
GWP-total kg CO2 eq. -1,10E+01 1,32E-01 5,49E-01 2,23E+00 3,37E-01 2,13E-03 7,49E-02 1,67E+01 6,00E-04 -9,67E-01
GWP-fossil kg CO2 eq. 2,94E+00 1,32E-01 5,92E-01 1,46E+00 4,26E-01 1,66E-03 7,47E-02 2,44E+00 5,93E-04 -5,98E-01
GWP-biogenic kg CO2 eq. -1,43E+01 3,58E-04 -5,85E-02 -6,25E-01 -1,24E-01 4,70E-04 2,01E-04 1,43E+01 6,90E-06 -3,67E-01
GWP-LULUC kg CO2 eq. 3,27E-01 5,83E-05 1,64E-02 1,39E+00 3,44E-02 3,42E-06 2,99E-05 3,92E-05 1,83E-07 -2,07E-03
ODP kg CFC11 eq. 4,75E-07 3,16E-08 2,73E-08 3,44E-07 5,62E-08 4,54E-11 1,73E-08 1,26E-08 2,95E-10 -6,49E-08
AP mol H⁺ eq. 3,31E-02 4,47E-04 1,90E-03 5,28E-02 3,86E-03 6,69E-06 2,12E-04 3,16E-03 5,34E-06 -5,71E-03
EP-freshwater kg P eq. 1,26E-03 1,00E-05 6,89E-05 1,45E-03 1,41E-04 1,28E-06 4,89E-06 6,05E-05 4,77E-08 -1,69E-04
EP-marine kg N eq. 8,46E-03 1,06E-04 5,28E-04 7,36E-03 1,06E-03 1,47E-06 4,31E-05 1,55E-03 1,89E-06 -2,08E-03
EP-terrestial mol N eq. 8,16E-02 1,16E-03 5,23E-03 3,65E-02 1,04E-02 1,63E-05 4,70E-04 1,69E-02 2,07E-05 -2,34E-02
POCP kg NMVOC eq. 2,89E-02 4,56E-04 1,76E-03 1,41E-02 3,54E-03 3,72E-06 1,81E-04 4,43E-03 6,05E-06 -6,05E-03
ADP-M&M kg Sb eq. 4,50E-05 3,75E-07 2,34E-06 3,70E-05 4,84E-06 2,26E-08 2,65E-07 4,35E-07 1,62E-09 -1,64E-05
ADP-fossil MJ 5,09E+01 2,10E+00 2,80E+00 4,61E+01 5,79E+00 2,38E-02 1,13E+00 1,02E+00 2,10E-02 -8,82E+00
WDP m³ 1,25E+00 8,57E-03 6,53E-02 3,42E+00 1,35E-01 2,82E-04 3,34E-03 2,45E-02 1,02E-04 -1,87E-01
GWP-total: Global Warming Potential; GWP-fossil: Global Warming Potential fossil fuels; GWP-biogenic: Global Warming Potential biogenic; GWP-LULUC: Global Warming
Potential land use and land use change; ODP: Depletion potential of the stratospheric ozone layer; AP: Acidification potential, Accumulated Exceedance; EP-freshwater:
Eutrophication potential, fraction of nutrients reaching freshwater end compartment; See “additional Norwegian requirements” for indicator given as PO4 eq. EP-marine:
Eutrophication potential, fraction of nutrients reaching freshwater end compartment; EP-terrestial: Eutrophication potential, Accumulated Exceedance; POCP: Formation
potential of tropospheric ozone; ADP-M&M: Abiotic depletion potential for non-fossil resources (minerals and metals); ADP-fossil: Abiotic depletion potential for fossil
resources; WDP: Water deprivation potential, deprivation weighted water counsumption
Additional environmental impact indicators
Indicator Unit A1-A3 A4 A5 B2 B3 C1 C2 C3 C4 D
PM Disease incidence 9,80E-07 1,36E-08 5,15E-08 2,23E-07 1,07E-07 3,84E-11 4,73E-09 2,49E-08 1,08E-10 -3,91E-07
IRP kBq U235 eq. 4,78E-01 1,09E-02 2,55E-02 3,01E-01 5,25E-02 4,15E-04 5,83E-03 4,41E-03 9,82E-05 -1,35E-01
ETP-fw CTUe 1,13E+02 1,77E+00 6,09E+00 1,10E+02 1,24E+01 4,09E-02 8,89E-01 3,18E+00 1,14E-02 -4,88E+01
HTP-c CTUh 1,22E-08 5,31E-11 3,12E-09 8,77E-09 5,16E-09 9,47E-13 2,86E-11 3,96E-08 2,71E-13 -1,02E-09
HTP-nc CTUh 1,36E-07 2,07E-09 8,22E-09 9,31E-08 1,57E-08 2,72E-11 8,98E-10 1,27E-08 5,43E-12 -3,50E-08
SQP Dimensionless 2,42E+03 2,91E+00 1,21E+02 9,09E+01 2,55E+02 2,90E-02 7,89E-01 3,09E-01 6,56E-02 -1,65E+02
PM: Particulate matter emissions; IRP: Ionising radiation, human health; ETP-fw: Ecotoxicity (freshwater); ETP-c: Human toxicity, cancer effects; HTP-nc: Human toxicity,
non-cancer effects; SQP: Land use related impacts / soil quality
EPD for the best environmental decision 8
Classification of disclaimers to the declaration of core and additional environmental impact indicators
ILCD classification Indicator Disclaimer
Global warming potential (GWP) None
ILCD type / level 1 Depletion potential of the stratospheric ozone layer (ODP) None
Potential incidence of disease due to PM emissions (PM) None
Acidification potential, Accumulated Exceedance (AP) None
Eutrophication potential, Fraction of nutrients reaching freshwater end compartment (EP-freshwater) None
Eutrophication potential, Fraction of nutrients reaching marine end compartment (EP-marine) None
ILCD type / level 2
Eutrophication potential, Accumulated Exceedance (EP-terrestrial) None
Formation potential of tropospheric ozone (POCP) None
Potential Human exposure efficiency relative to U235 (IRP) 1
Abiotic depletion potential for non-fossil resources (ADP-minerals&metals) 2
Abiotic depletion potential for fossil resources (ADP-fossil) 2
Water (user) deprivation potential, deprivation-weighted water consumption (WDP) 2
ILCD type / level 3 Potential Comparative Toxic Unit for ecosystems (ETP-fw) 2
Potential Comparative Toxic Unit for humans (HTP-c) 2
Potential Comparative Toxic Unit for humans (HTP-nc) 2
Potential Soil quality index (SQP) 2
Disclaimer 1 – This impact category deals mainly with the eventual impact of low dose ionizing radiation on human health of the nuclear fuel cycle. It does not consider effects due to
possible nuclear accidents, occupational exposure nor due to radioactive waste disposal in underground facilities. Potential ionizing radiation from the soil, from radon and from some
construction materials is also not measured by this indicator.
Disclaimer 2 – The results of this environmental impact indicator shall be used with care as the uncertainties on these results are high or as there is limited experienced with the indicator
EPD for the best environmental decision 9
Resource use
Parameter Unit A1-A3 A4 A5 B2 B3 C1 C2 C3 C4 D
RPEE MJ 4,69E+02 3,16E-02 2,35E+01 2,60E+00 4,93E+01 2,04E-02 1,62E-02 5,23E-02 5,63E-04 -5,90E+01
RPEM MJ 1,77E+02 0,00E+00 8,85E+00 4,39E-01 1,86E+01 0,00E+00 0,00E+00 0,00E+00 0,00E+00 0,00E+00
TPE MJ 4,70E+02 3,16E-02 2,35E+01 3,04E+00 4,93E+01 2,04E-02 1,62E-02 5,23E-02 5,63E-04 -5,90E+01
NRPE MJ 4,65E+01 2,10E+00 2,58E+00 2,61E+01 5,32E+00 2,38E-02 1,13E+00 1,02E+00 2,10E-02 -8,82E+00
NRPM MJ 3,53E+01 0,00E+00 1,76E+00 2,88E+00 3,70E+00 0,00E+00 0,00E+00 0,00E+00 0,00E+00 0,00E+00
TRPE MJ 4,71E+01 2,10E+00 2,61E+00 2,90E+01 5,39E+00 2,38E-02 1,13E+00 1,02E+00 2,10E-02 -8,82E+00
SM kg 2,96E-03 0,00E+00 1,48E-04 7,13E-03 3,10E-04 0,00E+00 0,00E+00 0,00E+00 0,00E+00 0,00E+00
RSF MJ 1,28E+01 0,00E+00 6,39E-01 1,62E-03 1,34E+00 0,00E+00 0,00E+00 0,00E+00 0,00E+00 0,00E+00
NRSF MJ 2,93E-05 0,00E+00 1,47E-06 1,32E-04 3,08E-06 0,00E+00 0,00E+00 0,00E+00 0,00E+00 0,00E+00
W m3 4,14E-01 2,79E-04 2,11E-02 1,75E+00 4,40E-02 6,25E-05 1,20E-04 4,86E-03 2,73E-05 -1,78E-01
RPEE Renewable primary energy resources used as energy carrier; RPEM Renewable primary energy resources used as raw materials; TPE Total use of renewable primary
energy resources; NRPE Non renewable primary energy resources used as energy carrier; NRPM Non renewable primary energy resources used as materials; TRPE Total use
of non renewable primary energy resources; SM Use of secondary materials; RSF Use of renewable secondary fuels; NRSF Use of non renewable secondary fuels; W Use of
net fresh water
End of life - Waste
Parameter Unit A1-A3 A4 A5 B2 B3 C1 C2 C3 C4 D
HW KG 2,84E-02 1,34E-04 5,32E-03 1,97E-02 8,79E-03 3,90E-06 5,82E-05 9,18E-04 5,68E-02 -5,73E-03
NHW KG 1,72E+00 2,43E-01 1,14E-01 2,03E+00 2,22E-01 1,59E-04 5,93E-02 8,15E-02 4,78E-02 -2,27E-01
RW KG 2,58E-04 1,41E-05 1,43E-05 1,44E-04 2,96E-05 1,04E-07 7,65E-06 2,51E-06 1,31E-07 -4,33E-05
HW Hazardous waste disposed; NHW Non hazardous waste disposed; RW Radioactive waste disposed
EPD for the best environmental decision 10
End of life – output flow
Parameter Unit A1-A3 A4 A5 B2 B3 C1 C2 C3 C4 D
CR kg 0,00E+00 0,00E+00 0,00E+00 0,00E+00 0,00E+00 0,00E+00 0,00E+00 0,00E+00 0,00E+00 0,00E+00
MR kg 2,01E-03 0,00E+00 2,01E-02 0,00E+00 2,21E-03 0,00E+00 0,00E+00 0,00E+00 0,00E+00 0,00E+00
MER kg 0,00E+00 0,00E+00 4,58E-01 0,00E+00 9,63E-01 0,00E+00 0,00E+00 0,00E+00 0,00E+00 0,00E+00
EEE MJ 2,82E-03 0,00E+00 1,41E-04 0,00E+00 2,96E-04 0,00E+00 0,00E+00 0,00E+00 0,00E+00 0,00E+00
ETE MJ 2,40E-02 0,00E+00 1,20E-03 0,00E+00 2,52E-03 0,00E+00 0,00E+00 0,00E+00 0,00E+00 0,00E+00
CR Components for reuse; MR Materials for recycling; MER Materials for energy recovery; EEE Exported electric energy; ETE Exported thermal energy
Reading example: 9,0 E-03 = 9,0*10-3 = 0,009
Information describing the biogenic carbon content at the factory gate
Biogenic carbon content Unit Value
Biogenic carbon content in product kg C 3,89
Biogenic carbon content in the accompanying packaging kg C 0
EPD for the best environmental decision 11
Additional Norwegian requirements
Greenhous gas emission from the use of electricity in the manufacturing phase
For the manufacturing process (A3 Superwood) 100% renewable electricity from Danish wind power
is used in calculations. The renewable sources of electricity are evidenced by Guarantee of Origin
certificates (Miljøvenlig El, Energi Danmark).
Guarantee of Origin is valid throughout the validity period of the EPD. Documentation on certificate
is provided upon request to Superwood A/S.
National production mix from import, low voltage (production of transmission lines, in addition to
direct emissions and losses in grid) for wind power electricity production.
For assembly (A5) and de-construction (C1) national market mix from import, low voltage
(production of transmission lines, in addition to direct emissions and losses in grid) is used.
National electricity grid Unit Value
Electricity, low voltage {DK, Guarantee of Origin: wind power, KlimaEl wind }|
kg CO2 -eq/kWh 0,022
market for | Cut-off, U – Ecoinvent (A3 Superwood)
Electricity, low voltage {DK}| market for | Cut-off, U – Ecoinvent (A5, C1) kg CO2 -eq/kWh 0,246
Additional GWP results calculations using the physical national electricity grid mix
(energy sources without a Guarantee of Origin)
Production (A3) of Superwood is calculated without the use of Guarantee of Origin (used DK market
mix).
National electricity grid Unit Value
Electricity, low voltage {DK}| market for | Cut-off, U – Ecoinvent (A5, C1) kg CO2 -eq/kWh 0,246
Indicator Unit A1-A3
GWP-total kg CO2 eq. -1,01E+01
GWP-fossil kg CO2 eq. 3,80E+00
GWP-biogenic kg CO2 eq. -1,43E+01
GWP-LULUC kg CO2 eq. 3,29E-01
Additional environmental impact indicators required in NPCR Part A for construction
products
In order to increase the transparency of biogenic carbon contribution to climate impact, the
indicator for GWP has been sub-divided into the following:
GWP-IOBC Climate impacts calculated according to the principle of instantanious oxidation
GWP-BC Climate impacts from the net uptake and emission of biogenic carbon from each module.
In addition, EP-freshwater shall also declared as PO4 eq.
EPD for the best environmental decision 12
Indicator Unit A1-A3 A4 A5 B2 B3 C1 C2 C3 C4 D
EP- kg PO4 7,93E- 6,30E- 8,62E- 1,17E- 4,60E- 3,65E- 3,11E- 8,84E- -1,59E-03
8,18E-03
freshwater* eq. 05 04 03 03 06 05 03 07
kg CO2 1,32E- 5,92E- 1,46E+ 4,26E- 1,66E- 7,47E- 2,44E+ 5,93E- -6,42E-01
GWP-IOBC 2,94E+00
eq. 01 01 00 01 03 02 00 04
kg CO2 0,00E+ 0,00E+ 0,00E+ 0,00E+ 0,00E+ 0,00E+ 1,43E+ 0,00E+ 0,00E+00
GWP-BC -1,43E+01
eq. 00 00 00 00 00 00 01 00
kg CO2 1,32E- 5,92E- 1,46E+ 4,26E- 1,66E- 7,47E- 1,67E+ 5,93E- -6,42E-01
GWP -1,13E+01
eq. 01 01 00 01 03 02 01 04
EP-freshwater* Eutrophication potential, fraction of nutrients reaching freshwater end compartment. Declared
as PO4 eq. GWP-IOBC Global warming potential calculated according to the principle of instantanious
oxidation. GWP-BC Global warming potential from net uptake and emissions of biogenic carbon from the
materials in each module. GWP Global warming potential
Hazardous substances
The declaration is based upon reference to threshold values and/or test results and/or material
safety data sheets provided to EPD verifiers. Documentation available upon request to EPD owner.
☒The product contains no substances given by the REACH Candidate list or the Norwegian
priority list.
☐The product contains substances given by the REACH Candidate list or the Norwegian
priority list that are less than 0,1 % by weight.
☐The product contain dangerous substances, more then 0,1% by weight, given by the REACH
Candidate List or the Norwegian Priority list, see table.
☐The product contains no substances given by the REACH Candidate list or the Norwegian
priority list. The product is classified as hazardous waste (Avfallsforskiften, Annex III), see
table.
Name CAS no. Amount
Indoor environment
Superwood is intended for external use and will not affect indoor environment.
EPD for the best environmental decision 13
Bibliography
ISO 14025:2010 Environmental labels and declarations - Type III environmental
declarations - Principles and procedures
ISO 14044:2006 Environmental management - Life cycle assessment - Requirements
and guidelines
EN 15804:2012+A2:2019 Sustainability of construction works - Environmental product
declaration - Core rules for the product category of construction
products
ISO 21930:2007 Sustainability in building construction - Environmental declaration of
building products
Andvik Dahlstrøm, Oddbjørn LCA-report for Superwood A/S. LCA-report nr 632284-26 EPD
Superwood from Asplan Viak AS, Sandvika, Norway, 2022
EPD-Norge 2021 NPCR Part A:2021 Construction products and services Ver 2
EPD-Norge 2021 NPCR 015 Part B for wood and wood-based products 4.0
DS/EN 335:2013 Durability of wood and wood-based products - Use classes:
definitions, application to solid wood and wood-based products
RTS_124_21 EPD Finnish sawn and planed timber
RTS_13_18 EPD Teknos Water-borne exterior paints
S-P-02150 EPD of Stora Enso Classic Sawn
NEPD-2546-1284-NO EPD Moelven sawn timber
NS-EN 16449:2014 Wood and wood-based products - Calculation of the biogenic carbon
content of wood and conversion to carbon dioxide
NS-EN 16485:2014 Round and sawn timber - Environmental Product Declarations -
Product category rules for wood and wood-based products for use in
construction
SSB (2020) Table 04727 District Heating Balance (GWh)
SSB (2020) Table 04730 Consumption of fuel for gross production of district heating, by
source of energy
SSB (2020) Table 09469 Net production of district heating, by heating system
Program Operator tlf +47 23 08 80 00
The Norwegian EPD Foundation
Post Box 5250 Majorstuen, 0303 Oslo e-post: post@epd-norge.no
Norway web www.epd-norge.no
Publisher tlf +47 23 08 80 00
The Norwegian EPD Foundation
Post Box 5250 Majorstuen, 0303 Oslo e-post: post@epd-norge.no
Norway web www.epd-norge.no
Owner of the declaration tlf +45 7687 3200
Superwood A/S
Palsgaardvej 3, DK-7362 Hampen e-post: smk@superwood.dk
Denmark web www. superwood.dk
Author of the life cycle assessment tlf +47 417 99 417
Asplan Viak AS, Oddbjørn Dahlstrøm Andvik
Kjørboveien 20, 1337 Sandvika e-post: oddbjorn.dahlstrom@asplanviak.no
Norway web www.asplanviak.no
EPD for the best environmental decision 14
EPD for the best
environmental
decision
The Norwegian EPD foundation
www.epd-norge.no
EPD for the best environmental decision 15
