ENVIRONMENTAL PRODUCT DECLARATION
as per ISO 14025 and EN 15804+A2
Owner of the Declaration FAAC
Programme holder Institut Bauen und Umwelt e.V. (IBU)
Publisher Institut Bauen und Umwelt e.V. (IBU)
Declaration number EPD­FAA­20220003­CBB1­EN
Issue date 12.04.2022
Valid to 11.04.2027
FAAC A952 Drive for swing doors
FAAC
www.ibu-epd.com | https://epd-online.com
Umwelt Produktdeklaration Name des Herstellers – Name des Produkts
General Information
FAAC FAAC A952 Drive for swing doors
Programme holder Owner of the declaration
IBU – Institut Bauen und Umwelt e.V. FAAC
Panoramastr. 1 Via Calari, 10
10178 Berlin 40069 Zola Predosa (BO)
Germany Italy
Declaration number Declared product / declared unit
EPD­FAA­20220003­CBB1­EN FAAC A952 Drive for swing doors
This declaration is based on the product Scope:
category rules: This declaration and its LCA study are related to one
Drive systems for automatic doors and gates, 11.2017 (1) FAAC A952 Drive for swing doors. The final
(PCR checked and approved by the SVR) assembly and production stage occur in Zola Predosa,
Bologna (Italy). Components are sourced from
international tier­one suppliers. The FAAC A952 Drive
Issue date
for swing doors is composed of operator unit, arms
12.04.2022
and, in some exceptional cases, the customer buys an
optional external battery back­up unit. The battery
Valid to back­up, having the same design and colour, is
11.04.2027 mounted as an extension of the main body of the drive.
This declaration only refers to the product without the
back­up battery unit (results with battery are visible in
the project report).
The owner of the declaration shall be liable for the
underlying information and evidence; the IBU shall not
be liable with respect to manufacturer information, life
cycle assessment data and evidences.
The EPD was created according to the specifications
of EN 15804+A2. In the following, the standard will be
simplified as EN 15804.
Verification
The standard EN 15804 serves as the core PCR
Independent verification of the declaration and data
according to ISO 14025:2010
Dipl. Ing. Hans Peters internally x externally
(chairman of Institut Bauen und Umwelt e.V.)
Dr. Alexander Röder Dr. Matthew Fishwick
(Managing Director Institut Bauen und Umwelt e.V.)) (Independent verifier)
Product
Product description/Product definition movements. The operator moves, with a 100% duty
The A952 is an automated swing door drive. Its cycle, a door with a 130 kg/m2 as a moment of inertia.
technology is electromechanical. An electrical motor A952 conforms to EN16005, meeting all requirements
opens the door and a spring closes it. During the for escape routes regulations EN13489­1.
closing phase, the motor controls the speed. Through
a programmed configuration, the opening and closing For the placing on the market in the European
speeds are selected in order to match the weight of the Union/European Free Trade Association (EU/EFTA)
door. The architecture of the product consists of an (with the exception of Switzerland) the following legal
electronic board acting as a control unit, the power provisions apply:
supply, while the mechanical part is integrated into a Directive:
unique block containing the motor, the reduction gear 2006/42/CE - DIRECTIVE 2006/42/EC OF THE
box and the spring. EUROPEAN PARLIAMENT AND OF THE COUNCIL
The drive can be connected to the door leaf using an of 17 May 2006 on machinery, and amending Directive
arm that the customer can choose, depending on its 95/16/EC (recast) (Text with EEA relevance)
application, between different options. 2014/30/UE - DIRECTIVE 2014/30/EU OF THE
The patented technology used in the reduction gear EUROPEAN PARLIAMENT AND OF THE COUNCIL
box, grants smooth and quietly open and close of 26 February 2014 on the harmonisation of the laws
2 Environmental Product Declaration FAAC – FAAC A952 Drive for swing doors
of the Member States relating to electromagnetic EN 60335-1:2012 + A11:2014 + A13:2017
compatibility (recast) (Text with EEA relevance) EN 60335-1:2013
2011/65/UE - DIRECTIVE 2011/65/EU OF THE EN ISO 13849-1:2015
EUROPEAN PARLIAMENT AND OF THE COUNCIL EN ISO 13849-2:2012
of 8 June 2011 on the restriction of the use of certain EN 60335-2-103:2015
hazardous substances in electrical and electronic EN 16005:2012
equipment (recast) (Text with EEA relevance) EN IEC 63000:2018
EN 61000-6-2:2005
EN standards: EN 61000-6-3:2007 + A1:2011
UNI EN ISO 12100:2010, Safety of machinery —
General principles for design — Risk assessment and Technical data & Performances
risk reduction Name Value Unit
EN 60335-1:2012 + A11:2014 + A13:2017, Household Height 74 mm
and similar electrical appliances - Safety - Part 1: Installation depth 150 mm
General requirements Length 715 mm
EN 60335-1:2013, , Household and similar electrical Anodized
Profile finish /
appliances - Safety - Part 1: General requirements alluminium
EN ISO 13849-1:2015 Cat 2PL c, Safety of machinery Weight (packaging excluded) 13.65 kg
— Safety-related parts of control systems — Part 1: 100­240
General principles for design Mains power supply Vac, 50­ /
EN ISO 13849-2:2012, Safety of machinery — Safety- 60Hz
related parts of control systems — Part 2: Validation Maximum power consumption 350 W
EN 60335-2-103:2015, Household and similar
Auxiliary voltage 24Vcc, 1A /
electrical appliances – Safety – Part 2: particular
Opening time (adjustable) 4­10 s
requirements for drives for gates, doors and windows
Closing time (adjustable) 4­10 s
EN 16005:2012, Power operated pedestrian doorsets
Hold open time 0­30 s
– Safety in use – Requirements and test methods
Ambient temperature ­20 / +45 °C
EN IEC 63000:2018, Technical documentation for the
Low
assessment of electrical and electronic products with
Energy,
respect to the restriction of hazardous substances
Full Energy
EN 61000-6-2:2005, Electromagnetic compatibility Impact forces /
with
(EMC) – Part 6-2: Generic standards – Immunity for
security
industrial environments
sensors
EN 61000-6-3:2007 + A1:2011, Electromagnetic
compatibility (EMC) – Part 6-3: Generic standards –
emission standard for residential, commercial and
light-industrial environments
The CE­marking takes into account the proof of
Base materials/Ancillary materials
conformity with the respective harmonized standards
based on the legal provisions above. For the
The average composition of FAAC A952 Drive for
application and use the respective national provisions
swing doors is as follows:
apply.
Name Value Unit
Application
Steel 38.8 %
The FAAC A952 electromechanical operator is
Zama 18.1 %
designed to operate pedestrian swing doors with
Aluminium 16.9 %
horizontal movement. The A952 is designed to
motorise standard entrances, escape routes, smoke Electric and electro mechanic 16.7 %
and/or fire doors. The A952 is suitable for indoor Brass 5.4 %
installation or outdoor installation if protected from the Electronics 2.0 %
elements. One operator must be installed on each leaf. Plastics 0.1 %
Other 1.9 %
Technical Data
FAAC A952 electromechanical operator complies with This product does not contain substances listed in the
the requirements of EN 60335­2­103:2015 on candidate list (date: 01.12.2021) exceeding 0.1
“Household and similar electrical appliances – Safety – percentage by mass.
Part 2: particular requirements for drives for gates,
doors and windows” and is tested according to the Reference service life
testing procedure described in EN 16005:2012. The
technical sheet contains detailed information The product has a reference service life of more than
concerning quality features and product 1.000.000 cycles and 10 years of standard daily use
characteristics. (with the recommended maintenance and service
program). For this EPD a lifetime of 10 years is
The product is not harmonised in accordance with the considered.
PCR but in accordance with other provisions for
harmonisation of the EU:
UNI EN ISO 12100:2010
3 Environmental Product Declaration FAAC – FAAC A952 Drive for swing doors
LCA: Calculation rules
Declared Unit process. Offcuts and scraps during the manufacturing
The declaration refers to 1 FAAC A952 Drive for swing process are directed to a recycling unit.
doors as specified in IBU Part B.
Declared unit Assumptions
Name Value Unit The following assumptions were made:
Declared unit 1 pce.  labels were all considered to be made of
paper;
 density of the lubricant considered is 0.90
g/cm3;
System boundary
Cradle to gate with options.  a pressure of 10 bar was considered for the
The following life cycle stages were considered: use of compressed air;
 the magnet was considered to be 50% cobalt
Production stage: based and 50% samarium;
· A1 – Raw material extraction and processing
 a distance of 100 km was considered for the
· A2 – Transport to the manufacturer and
transport of the material to the
· A3 – Manufacturing
disposal/recovery/recycling site (C2);
Construction stage:  for the use phase and end of life an European
· A4 ­ Transport from the gate to the site scenarios was considered;
· A5 – Packaging waste processing
 for the end­of­life percentages of the product
the following directive: “Directive 2012/19/EU
Use stage related to the operation of the building
of the European Parliament and of the
includes:
· B6 – Operational energy use Council of 4 July 2012 on waste electrical and
electronic equipment (WEEE)” requires that at
End­of­life stage: least 80% shall be prepared for re­use and re­
· C2 – Transport to waste processing cycled. However, European statistics on
· C3 – Waste processing for recycling
recovery rates suggest 47% recycling
· C4 – Disposal (landfill, waste for incineration).
percentage is more likely for WEEE, and was
used for this study (EUROSTAT STATISTICS
This includes provision of all materials, products and
energy, packaging processing and its transport, as well ON WEEE PRODUCTS, 2018).
as waste processing up to the end­of­waste state or
disposal of final residues.
Cut-off criteria
Module D:
The only cut­off applied in the study is the use of
· Declaration of all benefits and loads
lubricant/grease corresponding to just a few grams
during the entire product assembling and it has been
Comparability
excluded. All reported data were incorporated and
Basically, a comparison or an evaluation of EPD data
modelled using best available LCI data.
is only possible if all the data sets to be compared
were created according to EN 15804 and the building
Software and database
context, respectively the product­specific
The LCA model is created using the GaBi ts Software
characteristics of performance, are taken into account.
system for life cycle engineering, developed by
Sphera. The GaBi LCI database provides the life cycle
GaBi 10 background database was mainly used for
inventory data for several of the raw and process
the calculation.
materials obtained from the background system. The
most recent of the database was 2021 (v2021.2).
All primary data are collected for the year 2020. All
Production process
secondary data come from the GaBi 2021 databases
The primary manufacturing processes are made by tier
and are representative of the years 2019­2023.
one suppliers and the final manufacturing processes
for operator units occur in factory in Zola Predosa,
Data Quality
Italy. The profiles are machined, and surface treated
The data quality can be described as good. The
as anodized (externally). Other parts, such as
primary data collection has been done thoroughly, all
electronics, arrive from tier one suppliers in Ireland,
relevant flows are considered.
and the motor comes from China. The drive system is
finally assembled in Zola Predosa. The only machines
Allocation:
used on the assembly line are two presses and a
Background data allocation
screwdriver; the remaining assembly is done manually
Information about background data is documented in
by the operators. The operators are packed in
http://database­documentation.gabi­
cardboard boxes and forwarded to the installer who will
software.com/support/gabi/.
then provide the installation on­site to the end
customer. The certified quality management system,
Foreground data allocation
EN ISO 9001:2015, ensures high standards to all
4 Environmental Product Declaration FAAC – FAAC A952 Drive for swing doors
The overall production (in terms of assembled consumption has been metered during 1 piece of
products) of FAAC S.p.A. comprises further products product assembling and compressed air consumption
beside the product considered in this study, but no has been measured by means of the litres consumed
allocation was needed as thermal and electrical energy during the assembling.
refer to the declared product. In particular, electricity
LCA: Scenarios and additional technical information
Characteristic product properties Reuse, recovery and/or recycling potentials (D),
Information on biogenic Carbon relevant scenario information
Name Value Unit
Collected separately waste type
13.65 kg
Information on describing the biogenic Carbon (excluding packaging)
Content at factory gate Recycling aluminium 7.96 %
Name Value Unit Recycling steel 18.26 %
Biogenic Carbon Content in Recycling brass 0.07 %
0 kg C
product Recycling electric and electro
8.90 %
Biogenic Carbon Content in mechanic
0.411 kg C
accompanying packaging Recycling plastics 0.72 %
Recycling alloys 11.04 %
Health protection and Environmental protection
Transport from the gate to the site (A4) during the manufacturing process
Name Value Unit Compliant with safety law and no additional tests
Truck distance 1557.41 km are required
Capacity utilisation Truck 53 % Measures for reducing noise during the
Ferry distance 34.55 km manufacturing process. The assembly lines follow
Capacity utilisation ferry 70 % the legislation on safety at work. In the case of the
A952 Drive for swing doors assembly line machinery,
Assembly (A5) the noise produced by the line is low to the point of not
Name Value Unit requiring hearing protectors for the operator
Cardboard packaging 0.958 kg
PVC adhesive 0.001 kg
Indication of the product performance on
LDPE film 0.007 kg
unforeseen contact with water
Polyamide band 0.007 kg In the event of floods or water­related environmental
disasters, to date the product does not contain
substances that have an impact on water. However,
Packaging end of life disposal routes the operation of the product may be affected.
Name Value Unit
Paper/cardboard packaging to
82.9 % Indication of fire performance in the event of
recycling
unforeseen fire
Paper/cardboard packaging to
7.6 % Not applicable.
energy recovery
Paper/cardboard packaging to
9.5 %
landfill Performance in the event of unforeseeable
Plastic packaging to recycling 41.8 % mechanical destruction
Plastic packaging to energy No hazards are anticipated during mechanical
recovery 33.6 % destruction.
Plastic packaging to landfill 24.6 %
Souce: Eurostat 2018 Disposal
After having dismantled the product, disposal in
Reference service life compliance with the current waste disposal regulations
Name Value Unit is assumed to occur. Components and structural
Reference service life 10 a materials, batteries and electronic components must
not be disposed of together with household waste.
Operational energy use (B6) They must be taken to authorized disposal and
Name Value Unit recycling centers. A 80% collection rate is a target
Electricity consumption 702.3 kWh based on the WEEE directive that requires that at least
80% of product produced by specific company must be
End of life (C1-C4) collected for recycling. Even though, EUROSTAT
Name Value Unit statistics show that an average 47% is the real
Collected separately aluminum, collection rate that is used in the model. The product is
13.65 kg
steel, plastics, electronic, etc. disposed with the code EER 16.02.00
Recycling aluminum, steel,
6.42 kg
plastics, electronic, etc. Maintenance
Landfilling 7.24 kg A952 Drive for swing doors doesn’t require
maintenance in the sense of replacement of parts or
lubrication; however, the correct tightening of screws
5 Environmental Product Declaration FAAC – FAAC A952 Drive for swing doors
must be checked annually. It is essential that
maintenance is carried out on other components that
are connected to it such as cables, structures, frames.
6 Environmental Product Declaration FAAC – FAAC A952 Drive for swing doors
LCA: Results
Disclaimer: EP­­freshwater: This indicator has been calculated as “kg P eq” as required
in the characterization model(EUTREND model, Struijs et al., 2009b, as implemented in ReCiPe;
http://eplca.jrc.ec.europa.eu/LCDN/developerEF.xhtml).
DESCRIPTION OF THE SYSTEM BOUNDARY (X = INCLUDED IN LCA; ND = MODULE OR INDICATOR NOT
DECLARED; MNR = MODULE NOT RELEVANT)
BENEFITS AND
CONSTRUCTI LOADS
PRODUCT STAGE ON PROCESS USE STAGE END OF LIFE STAGE BEYOND THE
STAGE SYSTEM
BOUNDARIES
7 Environmental Product Declaration FAAC – FAAC A952 Drive for swing doors
lairetam
waR
ylppus tropsnarT
gnirutcafunaM
eht
morf
tropsnarT
etis
eht
ot
etag
ylbmessA esU
ecnanetniaM
riapeR
tnemecalpeR tnemhsibrufeR
ygrene
lanoitarepO esu
retaw
lanoitarepO esu
noitcurtsnoc­eD
noitilomed tropsnarT
gnissecorp
etsaW
lasopsiD ­esueR ­yrevoceR ­gnilcyceR laitnetop
A1 A2 A3 A4 A5 B1 B2 B3 B4 B5 B6 B7 C1 C2 C3 C4 D
X X X X X ND ND MNR MNR MNR X ND X X X X X
RESULTS OF THE LCA - ENVIRONMENTAL IMPACT according to EN 15804+A2: 1 piece of FAAC A952
Drive for swing doors (backup battery excluded)
Core Indicator Unit A1-A3 A4 A5 B6 C1 C2 C3 C4 D
GWP­total [kg CO2­Eq.] 6.60E+1 1.98E+0 1.84E+0 2.82E+2 0.00E+0 1.53E­1 ­2.67E­1 1.34E­1 ­1.92E+1
GWP­fossil [kg CO2­Eq.] 6.76E+1 1.96E+0 3.54E­2 2.79E+2 0.00E+0 1.51E­1 ­2.70E­1 1.19E­1 ­1.92E+1
GWP­biogenic [kg CO2­Eq.] ­1.61E+0 5.84E­3 1.80E+0 2.37E+0 0.00E+0 4.51E­4 7.62E­3 1.46E­2 ­8.03E­2
GWP­luluc [kg CO2­Eq.] 4.79E­2 1.59E­2 9.40E­5 3.95E­1 0.00E+0 1.23E­3 ­5.10E­3 2.97E­4 ­8.10E­3
ODP [kg CFC11­Eq.] 4.73E­10 3.85E­16 5.14E­17 6.68E­12 0.00E+0 2.97E­17 3.55E­13 4.24E­16 ­1.09E­10
AP [mol H+­Eq.] 3.26E­1 7.25E­3 1.12E­4 5.81E­1 0.00E+0 5.56E­4 ­3.52E­2 7.45E­4 ­7.75E­2
EP­freshwater [kg PO4­Eq.] 1.17E­4 5.79E­6 8.56E­7 7.49E­4 0.00E+0 4.47E­7 1.54E­6 4.68E­6 ­3.50E­5
EP­marine [kg N­Eq.] 5.26E­2 3.38E­3 5.25E­5 1.38E­1 0.00E+0 2.59E­4 ­1.16E­3 1.94E­4 ­1.21E­2
EP­terrestrial [mol N­Eq.] 5.68E­1 3.76E­2 5.02E­4 1.45E+0 0.00E+0 2.88E­3 ­1.20E­2 2.10E­3 ­1.30E­1
POCP [kg NMVOC­Eq.] 1.62E­1 1.23E­2 2.64E­4 4.11E­1 0.00E+0 5.09E­4 ­3.49E­3 2.80E­4 ­6.59E­2
ADPE [kg Sb­Eq.] 1.07E­2 1.73E­7 2.42E­9 8.21E­5 0.00E+0 1.33E­8 ­1.15E­3 1.05E­8 ­4.26E­3
ADPF [MJ] 8.81E+2 2.60E+1 3.20E­1 4.97E+3 0.00E+0 2.01E+0 4.76E+0 1.59E+0 ­2.40E+2
[m³ world­Eq
WDP 9.97E+0 1.81E­2 1.50E­2 4.48E+1 0.00E+0 1.40E­3 ­7.25E­1 9.91E­3 ­2.77E+0
deprived]
GWP = Global warming potential; ODP = Depletion potential of the stratospheric ozone layer; AP = Acidification potential of land and water; EP =
Caption Eutrophication potential; POCP = Formation potential of tropospheric ozone photochemical oxidants; ADPE = Abiotic depletion potential for non­
fossil resources; ADPF = Abiotic depletion potential for fossil resources; WDP = Water (user) deprivation potential
RESULTS OF THE LCA - INDICATORS TO DESCRIBE RESOURCE USE according to EN 15804+A2: 1 piece
of FAAC A952 Drive for swing doors (backup battery excluded)
Indicator Unit A1-A3 A4 A5 B6 C1 C2 C3 C4 D
PERE [MJ] 2.23E+2 1.49E+0 2.83E­2 2.29E+3 0.00E+0 1.15E­1 1.40E+0 1.94E­1 ­7.38E+1
PERM [MJ] 1.63E+1 0.00E+0 ­1.63E+1 0.00E+0 0.00E+0 0.00E+0 0.00E+0 0.00E+0 0.00E+0
PERT [MJ] 2.39E+2 1.49E+0 2.83E­2 2.29E+3 0.00E+0 1.15E­1 1.40E+0 1.94E­1 ­7.38E+1
PENRE [MJ] 8.75E+2 2.61E+1 3.21E­1 4.97E+3 0.00E+0 2.01E+0 4.76E+0 1.59E+0 ­2.41E+2
PENRM [MJ] 7.51E+0 0.00E+0 0.00E+0 0.00E+0 0.00E+0 0.00E+0 0.00E+0 0.00E+0 0.00E+0
PENRT [MJ] 8.83E+2 2.61E+1 3.21E­1 4.97E+3 0.00E+0 2.01E+0 4.76E+0 1.59E+0 ­2.41E+2
SM [kg] 1.39E+0 0.00E+0 0.00E+0 0.00E+0 0.00E+0 0.00E+0 0.00E+0 0.00E+0 0.00E+0
RSF [MJ] 0.00E+0 0.00E+0 0.00E+0 0.00E+0 0.00E+0 0.00E+0 9.73E­23 0.00E+0 ­1.15E­13
NRSF [MJ] 0.00E+0 0.00E+0 0.00E+0 0.00E+0 0.00E+0 0.00E+0 1.14E­21 0.00E+0 ­1.35E­12
FW [m³] 5.18E­1 1.71E­3 3.65E­4 2.23E+0 0.00E+0 1.32E­4 ­1.03E­2 3.14E­4 ­1.83E­1
PERE = Use of renewable primary energy excluding renewable primary energy resources used as raw materials; PERM = Use of
renewable primary energy resources used as raw materials; PERT = Total use of renewable primary energy resources; PENRE = Use of
non­renewable primary energy excluding non­renewable primary energy resources used as raw materials; PENRM = Use of non­
Caption
renewable primary energy resources used as raw materials; PENRT = Total use of non­renewable primary energy resources; SM = Use
of secondary material; RSF = Use of renewable secondary fuels; NRSF = Use of non­renewable secondary fuels; FW = Use of net fresh
water
RESULTS OF THE LCA – WASTE CATEGORIES AND OUTPUT FLOWS according to EN 15804+A2:
1 piece of FAAC A952 Drive for swing doors (backup battery excluded)
Indicator Unit A1-A3 A4 A5 B6 C1 C2 C3 C4 D
HWD [kg] 1.80E­6 1.37E­9 3.60E­11 1.31E­6 0.00E+0 1.06E­10 1.98E­8 1.94E­10 ­5.84E­8
NHWD [kg] 8.36E+0 4.09E­3 7.59E­2 3.52E+0 0.00E+0 3.16E­4 2.66E+0 6.58E+0 ­3.21E+0
RWD [kg] 4.27E­2 4.73E­5 6.14E­6 7.40E­1 0.00E+0 3.65E­6 1.51E­3 1.71E­5 ­1.32E­2
CRU [kg] 0.00E+0 0.00E+0 0.00E+0 0.00E+0 0.00E+0 0.00E+0 0.00E+0 0.00E+0 0.00E+0
MFR [kg] 0.00E+0 0.00E+0 7.99E­1 0.00E+0 0.00E+0 0.00E+0 7.40E+0 0.00E+0 0.00E+0
MER [kg] 0.00E+0 0.00E+0 0.00E+0 0.00E+0 0.00E+0 0.00E+0 0.00E+0 0.00E+0 0.00E+0
EEE [MJ] 0.00E+0 0.00E+0 2.17E­1 0.00E+0 0.00E+0 0.00E+0 0.00E+0 4.82E­3 0.00E+0
EET [MJ] 0.00E+0 0.00E+0 3.25E­1 0.00E+0 0.00E+0 0.00E+0 0.00E+0 0.00E+0 0.00E+0
HWD = Hazardous waste disposed; NHWD = Non­hazardous waste disposed; RWD = Radioactive waste disposed; CRU = Components
Caption for re­use; MFR = Materials for recycling; MER = Materials for energy recovery; EEE = Exported electrical energy; EET = Exported
thermal energy
RESULTS OF THE LCA – additional impact categories according to EN 15804+A2-optional:
1 piece of FAAC A952 Drive for swing doors (backup battery excluded)
Indicator Unit A1-A3 A4 A5 B6 C1 C2 C3 C4 D
[Disease
PM 3.76E­6 4.07E­8 7.63E­10 4.90E­6 0.00E+0 3.07E­9 ­2.87E­7 9.06E­9 ­7.98E­7
Incidence]
[kBq U235­
IRP 6.52E+0 6.92E­3 7.24E­4 1.21E+2 0.00E+0 5.34E­4 2.38E­1 1.95E­3 ­2.09E+0
Eq.]
ETP­fw [CTUe] 3.59E+2 1.93E+1 2.28E­1 2.09E+3 0.00E+0 1.49E+0 ­6.81E+0 5.28E+0 ­9.83E+1
HTP­c [CTUh] 6.42E­7 3.90E­10 7.54E­12 5.91E­8 0.00E+0 3.01E­11 1.56E­8 1.20E­10 ­1.78E­8
HTP­nc [CTUh] 1.12E­6 2.32E­8 6.91E­10 2.23E­6 0.00E+0 1.79E­9 1.82E­6 1.29E­8 ­6.56E­7
SQP [­] 1.53E+2 8.92E+0 6.74E­2 1.57E+3 0.00E+0 6.89E­1 ­1.02E+1 2.76E­1 ­2.43E+1
PM = Potential incidence of disease due to PM emissions; IR = Potential Human exposure efficiency relative to U235; ETP­fw = Potential
Caption comparative Toxic Unit for ecosystems; HTP­c = Potential comparative Toxic Unit for humans (cancerogenic); HTP­nc = Potential
comparative Toxic Unit for humans (not cancerogenic); SQP = Potential soil quality index
Disclaimer 1 – for the indicator “Potential Human exposure efficiency relative to U235”.
This impact category deals mainly with the eventual impact of low dose ionizing
radiation on human health of the nuclear fuel cycle. It does not consider effects due to possible
nuclear accidents, occupational exposure nor due to radioactive waste disposal in underground
facilities. Potential ionizing radiation from the soil, from radon and from some construction materials is also not
measured by this indicator.
Disclaimer 2 – for the indicators “abiotic depletion potential for non­fossil resources”, “abiotic depletion potential
for fossil resources”, “water (user) deprivation potential, deprivation­weighted water consumption”, “potential
comparative toxic unit for ecosystems”, “potential comparative toxic unit for humans – cancerogenic”, “Potential
comparative toxic unit for humans ­ not cancerogenic”, “potential soil quality index”.
The results of this environmental impact indicator shall be used with care as the
uncertainties on these results are high or as there is limited experienced with the indicator.
References
2006/42/CE EN 60335­2­103:2015, Household and similar
DIRECTIVE 2006/42/EC OF THE EUROPEAN electrical appliances – Safety – Part 2: particular
PARLIAMENT AND OF THE COUNCIL of 17 May requirements for drives for gates, doors and windows
2006 on machinery, and amending Directive 95/16/EC
(recast) (Text with EEA relevance) EN 61000­6­2
EN 61000­6­2:2005, Electromagnetic compatibility
2011/65/UE (EMC) – Part 6­2: Generic standards – Immunity for
DIRECTIVE 2011/65/EU OF THE EUROPEAN industrial environments
PARLIAMENT AND OF THE COUNCIL of 8 June 2011
on the restriction of the use of certain hazardous EN 61000­6­3
substances in electrical and electronic equipment EN 61000­6­3:2007 + A1:2011, Electromagnetic
(recast) (Text with EEA relevance) compatibility (EMC) – Part 6­3: Generic standards –
emission standard for residential, commercial and
2014/30/UE light­industrial environments
DIRECTIVE 2014/30/EU OF THE EUROPEAN
PARLIAMENT AND OF THE COUNCIL of 26 February EN IEC 63000
2014 on the harmonisation of the laws of the Member EN IEC 63000:2018, Technical documentation for the
States relating to electromagnetic compatibility (recast) assessment of electrical and electronic products with
(Text with EEA relevance) respect to the restriction of hazardous substances
EN 15804 EN ISO 13849­1
EN 15804:2019+A2, Sustainability of construction EN ISO 13849­1:2015 Cat 2PL c, Safety of machinery
works — Environmental Product Declarations — Core — Safety­related parts of control systems — Part 1:
rules for the product category of construction products. General principles for design
EN 16005 EN ISO 13849­2
EN 16005:2012, Power operated pedestrian doorsets EN ISO 13849­2:2012, Safety of machinery — Safety­
– Safety in use – Requirements and test methods related parts of control systems — Part 2: Validation
EN 60335­1 EN ISO 14040
EN 60335­1:2012 + A11:2014 + A13:2017, Household EN ISO 14040:2009­11 Environmental management ­
and similar electrical appliances ­ Safety ­ Part 1: Life cycle assessment ­ Principles and framework
General requirements
EN ISO 14044
EN 60335­2­103 EN ISO 14044:2006­10 Environmental management ­
Life cycle assessment ­ Requirements and guidelines
8 Environmental Product Declaration FAAC – FAAC A952 Drive for swing doors
GaBi ts
IBU 2021 GaBi ts dataset documentation for the software ­
General Instructions for the EPD programme of Institut system and databases, LBP, University of Stuttgart
Bauen und Umwelt e.V. Version 2.0, Berlin: Institut and Sphera, Leinfelden­Echterdingen, 2021
Bauen und Umwelt e.V., 2021. www.ibu­epd.com (http://documentation.gabi­software.com/)
IBU PART A REACH/ECHA candidate list
PCR ­ Part A: Calculation rules for the Life Cycle List of substances considered for authorisation
Assessment and Requirements on the Background substances of very high concern (SVHCs)
Report, version 1.2, Institut Bauen und Umwelt e.V., (ECHA candidate list), published in accordance with
www.bau­umwelt.com, 2013 Article 59, paragraph 10 of the REACH, Regulation
Helsinki: European Chemicals Agency, view of
IBU PART B 01.12.2021
PCR – Part B: Requirements of the EPD for Drive
systems for automatic doors and gates, version 1.6, UNI EN ISO 12100
Institut Bauen und Umwelt e.V., www.bau­umwelt.com, UNI EN ISO 12100:2010, Safety of machinery —
2013 General principles for design — Risk assessment and
risk reduction
ISO 14025
DIN EN ISO 14025:2011­10, Environmental labels and
declarations — Type III environmental declarations —
Principles and procedures.
9 Environmental Product Declaration FAAC – FAAC A952 Drive for swing doors
Publisher
Institut Bauen und Umwelt e.V. Tel +49 (0)30 3087748­ 0
Panoramastr. 1 Fax +49 (0)30 3087748­ 29
10178 Berlin Mail info@ibu­epd.com
Germany Web www.ibu-epd.com
Programme holder
Institut Bauen und Umwelt e.V. Tel +49 (0)30 ­ 3087748­ 0
Panoramastr 1 Fax +49 (0)30 – 3087748 ­ 29
10178 Berlin Mail info@ibu­epd.com
Germany Web www.ibu-epd.com
Author of the Life Cycle
Assessment Tel +49 711 341817­0
Sphera Solutions GmbH Fax +49 711 341817­25
Hauptstraße 111­ 113 Mail info@sphera.com
70771 Leinfelden­Echterdingen Web www.sphera.com
Germany
Owner of the Declaration
FAAC S.p.A. Soc. Unipersonale Tel +393516048828
Via Calari 10 Fax +390510957820
40069 Zola Predosa (BO) Mail
Italy alessandro.golfarelli@faacgroup.
com
Web www.faacgroup.com
