ENVIRONMENTAL PRODUCT DECLARATION
as per ISO 14025 and EN 15804+A2
Owner of the Declaration Adolf Würth GmbH & Co. KG
Publisher Institut Bauen und Umwelt e.V. (IBU)
Programme holder Institut Bauen und Umwelt e.V. (IBU)
Declaration number EPD-AWU-20230268-IBD1-EN
Issue date 12.09.2023
Valid to 12.09.2027
flexen® PE-Stabil
Adolf Würth GmbH & Co. KG
www.ibu-epd.com | https://epd-online.com
1. General Information
Adolf Würth GmbH & Co. KG flexen® PE-Stabil
Programme holder Owner of the declaration
IBU – Institut Bauen und Umwelt e.V. Adolf Würth GmbH & Co. KG
Hegelplatz 1 Reinhold-Würth-Str. 12-17
10117 Berlin 74653 Künzelsau
Germany Germany
Declaration number Declared product / declared unit
EPD-AWU-20230268-IBD1-EN flexen® PE-stabil
This declaration is based on the product category rules: Scope:
Insulating materials made of foam plastics, 01.08.2021 Product line flexen® PE-stabil Thermal insulation products for building
(PCR checked and approved by the SVR) equipment and
industrial insulations made of Polythene-based, closed-cell foam pipe
insulation with a robust protective coating (PEF) according to EN14313.
Issue date This declaration is an Environmental Product Declaration according to
ISO14025 describing the specific environmental performance of the
12.09.2023
product produced in Belgium at the site of Eynatten.
The owner of the declaration shall be liable for the underlying information
and evidence; the IBU shall not be liable with respect to manufacturer
Valid to
information, life cycle assessment data and evidences.
12.09.2027
The EPD was created according to the specifications of EN 15804+A2. In
the following, the standard will be simplified as EN 15804.
Verification
The standard EN 15804 serves as the core PCR
Independent verification of the declaration and data according to ISO
14025:2011
internally X externally
Dipl.-Ing. Hans Peters
(Chairman of Institut Bauen und Umwelt e.V.)
Florian Pronold Vito D'Incognito,
(Managing Director Institut Bauen und Umwelt e.V.) (Independent verifier)
1 Environmental Product Declaration - Adolf Würth GmbH & Co. KG - flexen® PE-Stabil
2. Product
(CMR) substances in categories 1A or 1B, which are not on the
2.1 Product description/Product definition candidate list, exceeding 0.1 percentage by mass: No.
flexen® PE-stabil is the Professional Biocide products were added to this construction product or it
Polythene-based closed-cell foam pipe insulation with has been treated with biocide products (this then concerns a
a robust PE protective coating for continuous energy treated product as defined by the (EU) Ordinance on Biocide
saving and condensation control purposes. Products No. 528/2012): No.
flexen® PE-stabil provides solutions that Name Value Unit
follow all necessary guidelines for any type of
LDPE 65.80 %
installation cf. PCR.
Flame retardant 1.9 %
For the placing on the market of the product in the
European Union/European Free Trade Association LLDPE 6.48 %
(EU/EFTA) (with the exception of Switzerland) - Internally recycled PE 14.73 %
Thermal Insulation products for building equipment and Pigment 2.42 %
industrial installations. Factory made polyethylene
Volume stabilizer 0.98 %
foam (PEF) and the CE-marking. For the application
Blowing Agent 7.69 %
and use, the respective national provisions apply.
PE and fillers give the aspect of the product. The blowing agent
2.2 Application causes the expansion during manufacturing and the flame
flexen® PE-stabil is used to insulate retardants ensure the fire resistance. According to the
pipes for heating and plumbing. European Chemicals Regulation REACH Manufacturers,
importers and downstream users must register their chemicals
• Polyethylene foam is a cost-efficient material
and are responsible for their safe use on their own. For its
with good insulating properties.
production the production plant uses exclusively verifiably
• Products made of PE foam yield an excellent
cost/performance ratio. registered and approved substances. flexen® PE-stabil does
• Heat loss control and noise reduction in fresh-and waste not contain Substances of Very High Concern (SVHC).
water and heating system Antimony trioxide and halogenated flame retardants
are applied.
2.3 Technical Data
Constructional data 2.6 Manufacture
Performance data of the product in accordance with The manufacturing process consists of a continuous extrusion.
the Declaration of Performance with respect to its Solid pellets of thermoplastic resin are fed to a melting zone in
Essential Characteristics according to EN 14313 apply. Further which the resin is melted, to form a
data: flowable thermoplastic mass. The thermoplastic mass is then
Name Value Unit metered to a mixing zone where the thermoplastic mass is
Gross density 26.7 kg/m3 thoroughly mixed with a blowing agent under pressure. The
mixture of thermoplastic resin and blowing agent is then forced
Thermal conductivity 0.04 W/(mK)
through a die,
Reaction To Fire Acc. to EN 13501-1
E which imparts a shape to the thermoplastic mass, into a zone of
depending on the thickness
lower pressure, such as atmospheric pressure. The blowing
Max Service Temperature Acc. To EN agent expands to form the cells of the foam and the
100 °C
14707 thermoplastic foam is cooled through an inline water cooler.
Min Service Temperature 0 °C The protection coating
water absorption Acc. to EN 13472 WS005 - "skin" is applied by co-extrusion. The "skin" is made with solid
pellets of thermoplastic resin and some additives, which is, with
traces quantities of water-soluble ions Cl < 20 – F < 4
- the help of an extruder, applied around the foam. There is not a
and pH-value Acc. to EN 13468 - pH 5,8
foaming agent used in this case. The die is positioned around
the
2.4 Delivery status
"naked" foam and deposes a small thickness (± 0.1mm) of PE
The PE products are supplied as tubes. The tubes are film on the foam. At the end of this process the profiles are cut
delivered in lengths of 2 m packed in cardboard boxes. The at dimension.
insulating sleeves in the flexen® PE-stabil have a thickness Quality assurance :
ranging from 4 to 25 mm and an inside diameter ranging from The manufacture is certified ISO 9001 for quality management.
15 to 42 mm. These products are categorized according to The product corresponds to the product standard EN 14313
thermal conductivity (Lambda*). The category of product with and has a Declaration of
lambda 0,040 (W/(mK)) (acc. to EN ISO 8497 and EN 12667). Performance according to the DOP no.
LE_0870609015_01_M_flexen_PE_Stabil
2.5 Base materials/Ancillary materials
(see www.wuerth.de)
Base materials
2.7 Environment and health during manufacturing
flexen® PE-stabil is a flexible insulation material based on
During all manufacturing steps the production follows the
Polyethylene with a protecting coating of PE, which consists of
national guidelines and regulations. Solar panels are installed
around 7 basic components. The following table displays the
on the roof of the warehouses.
different elements of the formula.
This product contains substances listed in the candidate list 2.8 Product processing/Installation
(date: 08.07.2021) exceeding 0.1 percentage by mass: No.
flexen® PE-stabil can be installed using
This product contains other carcinogenic, mutagenic, reprotoxic
basic tools like knives. No special tools or specific
2 Environmental Product Declaration - Adolf Würth GmbH & Co. KG - flexen® PE-Stabil
protection is necessary. When applying adhesives the recommended in EN16783.
information given in the relevant safety data sheets is Description of the influences on the ageing of the product when
to be heeded. The recommendations on how to use applied in accordance with the rules of technology.
the product are described in the application manuals or
videos. More details are listed on the Web Page
2.13 Extraordinary effects
WÜRTH (wuerth.de).
Fire
2.9 Packaging Fire According to flexen® PE-stabil are classified as EURO
flexen® PE-stabil products are packed in cardboard boxes and CLASS E and therefore have a
transported on reusable limited speed of inflammation.
pallets. The packaging material can be recycled. The pallets
Fire protection
used to transport the products are taken back or exchanged
Name Value
when the flexen® PE-stabil is delivered, so the use of pallets is
Building material class E
a closed loop economy.
2.10 Condition of use
Water
During the use of the product for the purpose for which they are flexen® PE-stabil are closed cell foam and obtain the better
intended, there are no modifications to the product during the
water absorption class WS005
use, except if due to extraordinary impact (see point 2.13).
according to the product standard
2.11 Environment and health during use
Mechanical destruction
There are no particular aspects of the material composition
flexen® PE-stabil are flexible foam covered with a PE protective
during the use. flexen® PE-stabil products are used in a wide
coating
range and variety of applications for which the product is
flexen® PE-stabil are not UV resistant. The use is not
intended. The PEF foams fulfil the German, Belgian and French
recommended for outside applications without complementary
regulations regarding the emission of VOC with emissions far
UV protection.
below the most severe limit values. The Eurofin Product Testing
institute, on the demand of the CEFEP (European group of PEF
2.14 Re-use phase
and FEF manufacturers) has made a wide range of tests for
In principle, if removed carefully, flexen® PE-stabil can be
different PEF products from different manufacturers. The
reused on any other piping system of similar dimensions. Any
insulation of heating pipes with allows a drastic reduction of
material not suitable for reuse is fully recyclable.
CO emission during the full service life of the installation. The
2
quantification of this is not in the topic of this EPD, and has to 2.15 Disposal
be evaluated in the frame of the LCA from the complete flexen® PE-stabil are fully recyclable using the same recycling
installation
systems as those used for
other forms of PE waste. Any non-recycled material should be
2.12 Reference service life
disposed of the materials according to the local regulations,
The function of flexen® PE-stabil is to ensure the insulation of
and by the European Waste Catalogue waste code 07 02 13
heating and sanitary
waste Plastic "Low Density Polyethylene"
installations for a reference service life (RSL) of 50 years. This
duration is based on the frequency of replacement of sanitary 2.16 Further information
and heating piping in buildings. Additional information about flexen® PE-stabil stabil can be
Although the insulation products are still effective after 50
found on the web site WÜRTH (wuerth.de). Here specification
years, it is assumed that when replacing the piping, the
clauses, data sheets and application manuals can be found.
insulation is not reused and is disposed of with the
piping. 50 years is the minimum Reference Service Life
3. LCA: Calculation rules
Name Value Unit
3.1 Declared Unit
Gross density 26.7 kg/m3
The declaration refers to 1 m³ of produced insulation product.
For the LCA calculations, as the product is foam and has some Declared unit 1 m3
tolerances, the density declared is the average between the Value for 1 m divided
Conversion factor from 1
product categories. The thermal conductivity coefficient section of the insulation pipe m
m³ to 1 linear meter
(Lambda-value) and R-value per 25 mm thickness per product ( m²)
brand is provided below as additional information and support Gross Density volume for
for installers 1 kg 0.02667 m³
Declared unit Thermal Conductivity at
0.040 W/(mK)
40°C
Thermal Conductivity λ: 0.040 W/mK at (40°C)
R-value- thickness: 25 mm: +/- 3,5 (m²K)/W
depending on the pipe diameter.
For IBU core EPDs (where clause 3.6 is part of the EPD): for
average EPDs, an estimate of the robustness of the LCA
values must be made, e.g. concerning the variability of the
production process, geographical representativeness and the
influence of background data and preliminary products
3 Environmental Product Declaration - Adolf Würth GmbH & Co. KG - flexen® PE-Stabil
compared to the environmental impacts caused by the actual The LCA calculation is conducted using the Gabi ts - database.
production. Not all necessary LCIs are included in the database. Where
data were missing or were unavailable or where suppliers were
unable to provide complete information, proxy datasets have
3.2 System boundary
been used.
The Data collection refers to the yearly production in 2021 The environmental burden for the production of pigments, flame
Module A1 to A3: retardants and volume stabilizers are approximated.
The LCA calculation covers the production of the raw materials,
transport of these to the plant, the mixing of raw materials 3.4 Cut-off criteria
according to the respective recipes, manufacturing of the foam Any glue and adhesive tapes used during the
product and packaging for dispatch. All production takes place installation (A5) have not been included as
exclusively in Eynatten, Belgium. quantification of these materials is uncertain and their
Module A4: use by the various installers is too diverse, adhesives
Transport of the final product to the application site. The and glues are not required in all/most cases, but may
average transport distance has be used for some applications.
been calculated based on a weighted value for the main In this study no others cut-off criteria have been
customers representing more than 91% of the sales volume in applied and all elementary incoming processes as well
2021. Capacity utilisation by volume is 100%. However, given as all energy and water inputs and waste outputs have
the low density of the product, capacity utilisation by mass has been counted.
been estimated as 10%.
Module A5: 3.5 Background data
The products can be placed end to end and the remaining The software system for life cycle engineering GaBi 2021 life
pieces can be reused on other cycle database used in the GaBi 10 software environment
pipes. The calculations do not contain any installation waste. (Service Pack 2021001000) developed by
Cardboard as a packaging material is assumed to be recycled. Thinkstep AG was used to perform this LCA.
As input material cardboard made of waste paper is
3.6 Data quality
considered. Thus, the environmental burden for packaging
material is considered already in A1-A3. The value of the All the foreground data requiring such energy or raw material
environmental impact for A5 is declared as '0'. coming from production, were verified and cross-checked
Module B1-B7: before being included in the model. Most of the life cycle
The foam insulation products do not require maintenance, inventories for the basic materials are contained in the GaBi 10
replacement or refurbishment software. For electrical and thermal energy Belgium-specific
while in use. The information modules B1 – B7 are not grid mixes and Belgium-specific supply for natural gas were
declared. Although the insulation flexen® PE-stabil contributes considered.
to a significant reduction of CO emissions from the heating or
2 3.7 Period under review
cooling equipment, this is not taken into account in this LCA. It
The production data for the year 2021 were used for the
should, however, be taken into account in the calculation of
realization of this study
environmental impacts of the complete heating and cooling
systems or of the complete building. 3.8 Geographic Representativeness
Module C1: Land or region, in which the declared product system is
As for the installation of the product, the disassembly is done manufactured, used or handled at the end of the product´s
manually and does not require any specific equipment. lifespan: Germany
Disassembly is generally carried out at the same time as the
replacement or removal of sanitary pipes. Consequently, there
are no 3.9 Allocation
impacts associated with C1. There is no co-product or by-product generated during the
Module C2:Transport at the end-of-life stage is modelled as a production. Due to the lack of specific data per production line
Euro Cargo 0-6 mix truck with diesel fuel. The average distance and product, the energy has been allocated per overall
to mechanical recycling is assumed to be 100 km. produced volume of insulation foam.
Module C3: Production waste
The legislation is pushing more in this direction and the overall Most of the production waste from the process (machine start,
pressure on plastic recycling is growing, the scenario with 100 end of production, non-conforming products, etc.) is recycled
% mechanical recycling is considered. The environmental internally in order to be reused in the manufacturing process.
burden is declared in module C3. These impacts are accounted for in A1-A3.
Module C4: The environmental burden for 100% landfilling is 0 Installation and End-of-Life waste
because 100 % mechanical recycling is considered. Installation of the foam products is done by hand and requires
Module D: The end-of-life scenarios for packaging material and no special equipment apart from a knife. Installation off-cut is
product do not deliver any benefits for the next system. not considered in this calculations. Any glue and adhesive
Recycling cardboard is a closed cycle with the production tapes used during the installation phase were not included in
process. The flexen® PE-stabil foam is fully recyclable and can the LCA
be
3.10 Comparability
used as a direct one-for-one substitute for virgin PE-LD
granulates, with only minor additive additions. Basically, a comparison or an evaluation of EPD data is only
possible if all the data sets to be compared were created
3.3 Estimates and assumptions according to EN 15804 and the building context, respectively
the product-specific characteristics of performance, are taken
into account.
4. LCA: Scenarios and additional technical information
4 Environmental Product Declaration - Adolf Würth GmbH & Co. KG - flexen® PE-Stabil
Characteristic product properties of biogenic carbon
The biogenic carbon content quantifies the amount of biogenic
Transport to the building site (A4)
carbon in a construction product leaving the factory gate, and it
shall be separately declared for the product and for any Name Value Unit
accompanying packaging. Litres of fuel 0.069 l/100km
If the total mass of biogenic carbon containing materials is less Transport distance 489 km
than 5 % of the total mass of the product and accompanying
Capacity utilisation (including empty runs) 10 %
packaging, the declaration of biogenic carbon content may be
Gross density of products transported 26.7 kg/m3
omitted. The mass of packaging containing biogenic carbon
shall always be declared.
Reference service life
Note: 1 kg of biogenic carbon is equivalent to 44/12 kg of CO2. Name Value Unit
Reference service life 50 a
Information on describing the biogenic Carbon Content at
End of life (C1-C4)
factory gate
Name Value Unit
Name ValueUnit
Recycling 26.7 kg
kg
Biogenic carbon content in product -
C
Biogenic carbon content in accompanying kg
5.58
packaging C
5 Environmental Product Declaration - Adolf Würth GmbH & Co. KG - flexen® PE-Stabil
5. LCA: Results
DESCRIPTION OF THE SYSTEM BOUNDARY (X = INCLUDED IN LCA; ND = MODULE OR INDICATOR NOT DECLARED; MNR =
MODULE NOT RELEVANT)
Benefits and
Construction loads beyond
Product stage Use stage End-of-life stage
process stage the system
boundaries
la ire ta m w a Ry lp p u s tro p s n a rT g n iru tc a fu n a M e h t m o rf tro p s n a rTe tis e h t o t e ta g y lb m e s s A e s U e c n a n e tn ia M ria p e R tn e m e c a lp e R tn e m h s ib ru fe R y g re n e la n o ita re p Oe s u re ta w la n o ita re p Oe s u n o itc u rts n o c -e Dn o itilo m e d tro p s n a rT g n is s e c o rp e ts a W la s o p s iD -e s u e R-y re v o c e R-g n ilc y c e Rla itn e to p
A1 A2 A3 A4 A5 B1 B2 B3 B4 B5 B6 B7 C1 C2 C3 C4 D
X X X X X MND MND MNR MNR MNR MND MND MND X X X X
RESULTS OF THE LCA - ENVIRONMENTAL IMPACT according to EN 15804+A2: 1 m³ flexen® PE-stabil
Parameter Unit A1-A3 A4 A5 C2 C3 C4 D
GWP-total kg CO 2 eq 1.02E+02 2.44E+00 0 2.27E-01 2.93E+00 0 -6.75E+01
GWP-fossil kg CO 2 eq 1.02E+02 2.45E+00 0 2.28E-01 2.89E+00 0 -6.7E+01
GWP-biogenic kg CO 2 eq -2.94E-01 -3.09E-02 0 -2.23E-03 4.03E-02 0 -5.72E-01
GWP-luluc kg CO 2 eq 1.41E-01 2.19E-02 0 1.54E-03 1.12E-03 0 -9.29E-03
ODP kg CFC11 eq 3.52E-08 3.07E-13 0 2.24E-14 1.19E-10 0 -4.1E-10
AP mol H+ eq 2.34E-01 2.88E-03 0 2.7E-04 4.14E-03 0 -9.3E-02
EP-freshwater kg P eq 4.35E-04 8.63E-06 0 8.14E-07 1.93E-05 0 -1.26E-04
EP-marine kg N eq 5.16E-02 9.78E-04 0 9E-05 1.65E-03 0 -2.72E-02
EP-terrestrial mol N eq 5.4E-01 1.15E-02 0 1.07E-03 1.67E-02 0 -2.84E-01
kg NMVOC
POCP 1.9E-01 2.94E-03 0 2.72E-04 4E-03 0 -8.88E-02
eq
ADPE kg Sb eq 1.04E-01 1.55E-07 0 2.3E-08 1.68E-06 0 -1.7E-05
ADPF MJ 3.41E+03 3.22E+01 0 2.99E+00 8.68E+01 0 -2.58E+03
m3 world eq
WDP 5.78E+00 2.85E-02 0 2.55E-03 2.09E-01 0 -1.14E+00
deprived
GWP = Global warming potential; ODP = Depletion potential of the stratospheric ozone layer; AP = Acidification potential of land and water; EP =
Eutrophication potential; POCP = Formation potential of tropospheric ozone photochemical oxidants; ADPE = Abiotic depletion potential for non-fossil
resources; ADPF = Abiotic depletion potential for fossil resources; WDP = Water (user) deprivation potential)
RESULTS OF THE LCA - INDICATORS TO DESCRIBE RESOURCE USE according to EN 15804+A2: 1 m³ flexen® PE-stabil
Parameter Unit A1-A3 A4 A5 C2 C3 C4 D
PERE MJ 4.49E+02 2.34E+00 0 2.07E-01 5.35E+01 0 -1.93E+02
PERM MJ 0 ND ND ND ND ND ND
PERT MJ 4.49E+02 2.34E+00 0 2.07E-01 5.35E+01 0 -1.93E+02
PENRE MJ 1.99E+03 3.23E+01 0 3E+00 8.68E+01 0 -2.58E+03
PENRM MJ 1.44E+03 ND ND ND ND ND ND
PENRT MJ 3.43E+03 3.23E+01 0 3E+00 8.68E+01 0 -2.58E+03
SM kg 1.38E+01 ND ND ND ND ND ND
RSF MJ 0 ND ND ND ND ND ND
NRSF MJ 0 ND ND ND ND ND ND
FW m3 5.26E-01 2.56E-03 0 2.4E-04 2.45E-02 0 -3.06E-01
PERE = Use of renewable primary energy excluding renewable primary energy resources used as raw materials; PERM = Use of renewable primary
energy resources used as raw materials; PERT = Total use of renewable primary energy resources; PENRE = Use of non-renewable primary energy
excluding non-renewable primary energy resources used as raw materials; PENRM = Use of non-renewable primary energy resources used as raw
materials; PENRT = Total use of non-renewable primary energy resources; SM = Use of secondary material; RSF = Use of renewable secondary fuels;
NRSF = Use of non-renewable secondary fuels; FW = Use of net fresh water
RESULTS OF THE LCA – WASTE CATEGORIES AND OUTPUT FLOWS according to EN 15804+A2:
1 m³ flexen® PE-stabil
Parameter Unit A1-A3 A4 A5 C2 C3 C4 D
HWD kg 4.07E-04 1E-10 0 1.59E-11 9.17E-09 0 -2.41E-07
NHWD kg 2.75E+00 4.92E-03 0 4.89E-04 1.15E-01 0 -7.13E-01
RWD kg 1.1E-01 6.04E-05 0 5.58E-06 2.02E-02 0 -2.16E-02
CRU kg 0 ND ND ND ND ND ND
MFR kg 0 ND 1.38E+01 ND 3.75E+01 ND ND
MER kg 0 ND ND ND ND ND ND
EEE MJ 0 ND ND ND ND ND ND
EET MJ 0 ND ND ND ND ND ND
HWD = Hazardous waste disposed; NHWD = Non-hazardous waste disposed; RWD = Radioactive waste disposed; CRU = Components for re-use;
MFR = Materials for recycling; MER = Materials for energy recovery; EEE = Exported electrical energy; EET = Exported thermal energy
6 Environmental Product Declaration - Adolf Würth GmbH & Co. KG - flexen® PE-Stabil
RESULTS OF THE LCA – additional impact categories according to EN 15804+A2-optional:
1 m³ flexen® PE-stabil
Parameter Unit A1-A3 A4 A5 C2 C3 C4 D
Disease
PM 7.43E-06 2.17E-08 0 2.06E-09 3.3E-08 0 -6.99E-07
incidence
IR kBq U235 eq 9.2E+00 9.01E-03 0 8.42E-04 1.4E+00 0 -2.14E+00
ETP-fw CTUe 1.74E+03 2.28E+01 0 2.12E+00 3.37E+01 0 -1.23E+03
HTP-c CTUh 4.27E-08 4.67E-10 0 4.37E-11 8.32E-10 0 -3.02E-08
HTP-nc CTUh 2.48E-06 2.51E-08 0 2.4E-09 2.58E-08 0 -1.41E-06
SQP SQP 2.92E+02 1.34E+01 0 1.27E+00 5.45E+01 0 -1.32E+02
PM = Potential incidence of disease due to PM emissions; IR = Potential Human exposure efficiency relative to U235; ETP-fw = Potential comparative
Toxic Unit for ecosystems; HTP-c = Potential comparative Toxic Unit for humans (cancerogenic); HTP-nc = Potential comparative Toxic Unit for humans
(not cancerogenic); SQP = Potential soil quality index
This EPD was created using a software tool.
6. LCA: Interpretation
The use of internal recycled material in flexen® PE-stabil almost 96% of the impact Global Warming Potential. As the
reduces the need for raw materials and avoids wasting flexen® PE-stabil is fully recyclable; the choice for the end of
resources. flexen® PE-stabil has a very low life was that of 100% recycling. This avoids the use of new raw
density, which means that little raw material is needed for high materials and or the exploitation of renewable or non-
insulation renewable resources. The end of life in 100% landfill has a
efficiency, which results in significant energy savings. In slight impact, especially from the point of view of climate
addition, flexen® PE-stabil is largely made of low-density change. However, the 100% incineration scenario has the
polyethylene, so it is fully recyclable and can be recycled when greatest impact because during incineration there is a
it reaches the end of its life. As there is a variation in density significant release of carbon dioxide. The insulation with
between the different references of the flexen® PE-stabil range, flexen® PE-stabil of the sanitary and heating piping contributes
a sensitivity analysis has been performed. The results of the to a significant reduction of CO 2 emissions from the heating or
LCA are given for 1m3 of product calculated with an average cooling equipment, this is not considered in this LCA. It should,
weighted foam density of 26.7 kg/m³. For the lowest density, the however, be taken into account in the calculation of
impacts are lowered by 13.9% and for the highest density the environmental impacts of the complete heating and cooling
impacts should be majored by 31.1%.However, these maximum systems or of the complete building.
densities of 33 and 35 kg/m³ only represent 4 references One way to continue to reduce the environmental impact of the
produced and sold in rather low volumes, and the same is true flexen® PE-stabil would be to continue to diversify our energy
for the lowest density of 23 kg/m³, which only represents 2 sources by switching more and more to renewable energies. To
references in the flexen® PE-stabil range. Most references are this end, after having greatly increased the number of
very close to the average density, but all impact factors can be photovoltaic panels, The Production plant will acquire a
recalculated based on their density. When we analyse the cogeneration system. Looking for more eco-responsible
complete life cycle, we see that the most impacting part for all suppliers must also be put in place, as well as finding raw
environmental impact factors is the production module and materials manufactured locally to avoid long-distance transport
more particularly the raw materials part. With regard to global as much as
warming for the complete life cycle, more than 95% comes from possible. An analysis of the plant's carbon footprint, which is
the production module 1,4% from transport to the places of currently being carried out, should identify areas for
installation and 3% comes from the end of life. A more in-depth improvement and find solutions to achieve the goal of zero
analysis of the production module A1 to A3 shows that the carbon.
production of raw materials and their transport account for
7. Requisite evidence
7.1. VOC emissions after 28 days. Certificates are available on request. 7.1 VOC
Eurofins Product Testing A/S has tested a wide range and emissions
variety of typical PEF (Polyethylene foam) products marketed in For products used in indoor applications.
the EU from CEFEP (European Test procedure to AgBB diagram indicating the measuring
Group of PEF/FEF manufacturers) Based on the loading factor agency, date and results as a range of values. At least the
0.05m²/m3 following must be declared:
(determined after consideration of the real-life applications of 7.2 Leaching
PEF products (in living rooms) and recommendations by the According to EN 13468 the content of water-soluble chloride
experts of the test institute) all results were found to be clearly ions for flexen® PE-stabil is
below the limit values. For all samples below 100mg/m3 TVOC <20mg/kg
8. References
EN 1602 EN ISO 8497: Thermal insulation - Determination of
EN 1602: 2013: Thermal insulating products for steady-state thermal transmission properties of thermal
building applications - Determination of the apparent insulation for circular pipes
density
ISO 9001
EN ISO 8497 ISO 9001: 2015: Quality management systems.
7 Environmental Product Declaration - Adolf Würth GmbH & Co. KG - flexen® PE-Stabil
EN 13472 Candidate List Substances of Very High Concern
EN 13472: Thermal insulating products for SVCH: date: 08.07.2021) exceeding 0.1 percentage by
building equipment and industrial installations - Determination mass
of short term
water absorption by partial immersion of preformed pipe
insulation CEFEP
CEFEP: European group of PEF and FEF manufacturers
EN 13468
EN 13468: Thermal insulating products for building Eurostat
equipment and industrial installations - Determination of trace European Statistics: Recovery rates for packaging
quantities of waste Paper and cardboard packaging for the
water-soluble chloride, fluoride, silicate, and sodium ions and European Union 27 countries 2014
pH http://ec.europa.eu/eurostat/home
Eurofins
EN 13501-1 Eurofins: Eurofins Scientific is a group of
EN 13501-1:2007+A1: 2013 Fire classification of international life sciences companies which provide a unique
construction products and building elements - range of
Classification using test data from reaction to fire tests analytical testing services to clients across multiple industries,
http://www.eurofins.com
ISO 14001
ISO 14001: 2015 Environmental management European Waste Catalogue
systems. European Waste Catalogue: waste code 07 02 13 waste Plastic
"Low Density Polyethylene"
EN ISO 14025
EN ISO 14025: 2011-10: Environmental labels and Gabi ts
declarations — Type III environmental declarations — GaBi 10 GaBi Software-System and Database for Life
Principles and procedures Cycle Engineering Copyright © 1992-2021 Sphera
Solutions Gmbh Version: 10.5.0.78 DB Schema 8007
ISO 14040
ISO 14040: Environmental management — Life cycle Institut Bauen und Umwelt
assessment — Principles and framework Institut Bauen und Umwelt e.V., Berlin(pub.): General
Instructions for the EPD Programme of Institut Bauen
ISO 14044 und Umwelt e.V., Version 2.0 2021.
ISO 14044: Environmental management — Life cycle
assessment — Requirements and guidelines Product Category Rules for Building-Related
Products and Services
EN 14707 Institute Construction and Environment e.V. (IBU)
EN 14707: 2012: Thermal insulating products for Part A: Calculation Rules for the Life Cycle
building equipment and industrial installations. Assessment and Requirements on the Project Report
Determination of maximum service temperature for Version 1.7
preformed pipe insulation
PCR Guidance-Texts for Building-Related Products
EN 15804 and Services
EN 15804: 2012-04 + A1 2014: Sustainability of From the range of Environmental Product Declarations
construction works — Environmental Product of Institute Construction and Environment e.V. (IBU)
Declarations — Core rules for the product category of Part B: Requirements on the EPD for Insulating
construction products materials made of foam plastics
Version 1.6 (Template) Version 1.2 (PCR specific)
CEN/TR 15941
CEN/TR 15941: Sustainability of construction works - REACH
Environmental product declarations - Methodology for According the European Chemicals
selection and use of generic data Regulation REACH manufacturers, importers and downstream
users must
CEN TS 16516 register their chemicals and are responsible for their safe use.
CEN TS 16516: AgBB, ISO 16000-3, /ISO 16000-6/,
/ISO16000-9/, /ISO 16000-11/ Construction products -
Assessment of release of dangerous substances. Sphera
Determination of emissions into indoor air Sphera Solutions Gmbh. GaBi 10 LCI documentation.
GaBi Databases (sphera.com) Stuttgart
EN 16783: 2017 The literature referred to in the Environmental Product
EN 16783: 2017 Thermal insulation products - Product Declaration must be listed in full.Standards already fully quoted
category rules (PCR) for factory made and in-situ in the EPD do not need to be listed here again.
formed products for preparing environmental product The current version of PCR Part A and PCR Part B of the PCR
declarations document on which they are based must be referenced.
8 Environmental Product Declaration - Adolf Würth GmbH & Co. KG - flexen® PE-Stabil
Publisher
Institut Bauen und Umwelt e.V. +49 (0)30 3087748- 0
Hegelplatz 1 info@ibu-epd.com
10117 Berlin www.ibu-epd.com
Germany
Programme holder
Institut Bauen und Umwelt e.V. +49 (0)30 3087748- 0
Hegelplatz 1 info@ibu-epd.com
10117 Berlin www.ibu-epd.com
Germany
Author of the Life Cycle Assessment
Owner of the Declaration
Adolf Würth GmbH & Co. KG +49 7940/15-0
Reinhold-Würth-Str. 12-17 info@wuerth.com
74653 Künzelsau www.wuerth.de
Germany
9 Environmental Product Declaration - Adolf Würth GmbH & Co. KG - flexen® PE-Stabil
