ENVIRONMENTAL PRODUCT DECLARATION
as per ISO 14025 and EN 15804+A2
Owner of the Declaration Pittsburgh Corning Europe NV
Programme holder Institut Bauen und Umwelt e.V. (IBU)
Publisher Institut Bauen und Umwelt e.V. (IBU)
Declaration number EPD-PCE-20200301-IBA1-EN
Issue date 24.02.2021
Valid to 23.02.2026
FOAMGLAS ® F
Pittsburgh Corning Europe NV
www.ibu-epd.com | https://epd-online.com
Umwelt Produktdeklaration Name des Herstellers – Name des Produkts
1. General Information
Pittsburgh Corning Europe NV FOAMGLAS® F
Programme holder Owner of the declaration
IBU – Institut Bauen und Umwelt e.V. Pittsburgh Corning Europe NV
Panoramastr. 1 Albertkade 1
10178 Berlin B-3980 Tessenderlo
Germany Belgium
Declaration number Declared product / declared unit
EPD-PCE-20200301-IBA1-EN FOAMGLAS® F / declared unit 1 kg uncoated cellular
glass insulation material
This declaration is based on the product Scope:
category rules: This document refers to the production of 1 kg
Mineral insulating materials, 12.2018 uncoated "FOAMGLAS® F" cellular glass
(PCR checked and approved by the SVR) manufactured in Belgium at the Tessenderlo
production facility of Pittsburgh Corning Europe NV.
The reference year of production is 2019. The
Issue date
environmental impacts of the coated product
24.02.2021
"FOAMGLAS® F in boards & blocks" are to be
assessed with the help of a markup factor in the
Valid to amount of 0.8% for Global Warming Potential. Besides
23.02.2026 FOAMGLAS® F, exclusively for building equipment
and industrial applications FOAMGLAS® HLB1600 has
the same environmental impacts as F.
The owner of the declaration shall be liable for the
underlying information and evidence; the IBU shall not
be liable with respect to manufacturer information, life
cycle assessment data and evidences.
The EPD was created according to the specifications
of EN 15804+A2. In the following, the standard will be
simplified as EN 15804.
Verification
The standard EN 15804 serves as the core PCR
Independent verification of the declaration and data
according to ISO 14025:2010
Dipl. Ing. Hans Peters internally x externally
(chairman of Institut Bauen und Umwelt e.V.)
Dr. Alexander Röder Matthias Klingler
(Managing Director Institut Bauen und Umwelt e.V.)) (Independent verifier)
2. Product
2.1 Product description/Product definition Trade Association (EU/EFTA) (with the exception of
FOAMGLAS® F is an insulation product for buildings Switzerland) Construction Products Regulation (CPR)
made of cellular glass. It is applied to the desired applies. The product declaration of performance (DOP)
dimensions in the form of slabs, panels, or other is taking into consideration EN 13167:2015 Thermal
specific elements. The FOAMGLAS® F is in general insulation products for buildings – Factory made
unfaced as a slab. In some cases, depending on the cellular glass (CG) products – Specification but also
end-use, the slabs can be faced with bitumen on the EN14305:2013 Thermal insulation for building
top with a PE-foil (e.g. READY, BOARDS) or a white equipment and industrial installations - Factory made
mineral liner (ROOFBLOCK, ROOF BOARDS). Also, cellular glass (CG) products – Specification.
on the bottom, the white mineral liner can be applied In addition to the common applications, especially for
(cf. BOARDS). loadbearing constructions and perimeter insulation, the
product also complies with the characteristics declared
The product is declared with a density of 165 kg/m³ in European Technical Assessment (ETA)
(±10%) and is supplied in thicknesses of 40 mm to 180 20/0221:2020 Cellular glass boards as load bearing
mm. layer and thermal insulation outside the waterproofing
and the CE-marking.
For the placing on the market of the product
FOAMGLAS® F in the European Union/European Free
2 Environmental Product Declaration Pittsburgh Corning Europe NV – FOAMGLAS® F
For the application and use the respective national FOAMGLAS® F are available in the following
provisions apply. dimensions:
- Slabs & Blocks: 600x450mm; 300x450mm
2.2 Application - Boards: 1200x600mm
FOAMGLAS® F products are used for roof, floors, Other dimensions are available on request.
loadbearing, perimeter or specific other insulation.
FOAMGLAS® F is also used for building equipment & 2.5 Base materials/Ancillary materials
industrial installations, for which FOAMGLAS® The main constituents of the product or its
HLB1600 is an equivalent product components are:
- Sand 15%
2.3 Technical Data - Feldspar 20%
The technical specifications of FOAMGLAS® F within - Recycled content (glass/scrap) 50% to 60%
the scope of this EPD and within the CE marking is - Others 5% to 15%
according to EN 13167, EN 14305 and ETA 20/0221.
1) This product/article/at least one partial article
In addition to the EN13167 declared values, the contains substances listed in the ECHA candidate list
characteristics declared for service temperature (- (date: 19.01.2021) exceeding 0.1 percentage by mass:
265°C – 430°C), thermal conductivity ranges & no
chloride content are in line with EN 14305. The same
for the ETA 20/0221 declared values on the 2) This product/article/at least one partial article
mechanical properities. Performance data of the contains other CMR substances in categories 1A or 1B
product in accordance with the declaration of which are not on the candidate list, exceeding 0.1
performance with respect to its essential percentage by mass: no
characteristics according to EN 13167.
3) Biocide products were added to this construction
Voluntary data: CEN KEYMARK certificate n°001-BK- product or it has been treated with biocide products
516-001; ATG H539; KOMO-CTG100-9; SIA CH672- (this then concerns a treated product as defined by the
13; ACERMI 023/253; Natureplus n°Zt-PCE-0406- (EU) Ordinance on Biocide Products No. 528/2012):
1101-101 no
Technical data according EN 13167 2.6 Manufacture
Name Value Unit The product is made following the protocol of the
Thermal conductivity λD 0.05 W/(mK) company. All glass constituents (recycled glass, sand,
Water vapour diffusion resistance ∞ sodium carbonate, feldspar, sodium sulfate, sodium
-
factor µ = ∞ (infinite being > 40000) (infinite) nitrate, iron oxide, and FOAMGLAS®-scrap) are melted
Gross density 165 kg/m3 (at ca. 1250°C) in the furnace and drawn into the
Compressive strength 1.6 N/mm2 shape of a thin-walled tube to enable efficient grinding.
Reaction to fire Class A1 Melted glass from the melter furnace is put in grinders
Dimensional stability at 70°C/95%RH to produce fine glass powder. In the grinding process,
DS70/90 ≤0.5mm additives are added so that afterwards, glass foaming
Water absorption (short/long) ≤ 0.5 kg/m² processes can be envisaged. In the foaming furnace,
cellular glass blocks are made in moulds by heating
Point load PL ≤ 1.0 mm
(sintering towards ca 850°C) the glass powder after the
BS ≥
Bending Strength kPa grinding process. After the foaming process, the
550
annealing process starts by moving the foamed blocks
CC(1.5/1
Compressive creep (long behaviour) kPa on the lehr where they cool according to a precisely
/50)600
determined curve. The cooled blocks are cut into
rectangular blocks and if necessary, ground or cut to
thinner sizes. The produced material is released,
labelled, marked, and packed for commercialisation
and various end-use applications (floor, roof, wall and
2.4 Delivery status
other construction elements).
FOAMGLAS® F are available in the following
thicknesses : from 40 to 180 mm
3 Environmental Product Declaration Pittsburgh Corning Europe NV – FOAMGLAS® F
1 Mixing and batching of the raw materials: Recycled 10 The FOAMGLAS® blocks pass through an
glass, feldspar, sodium carbonate, iron oxide, annealing oven to allow carefully controlled cooling
manganese oxide, sodium sulphate, sodium nitrate. without thermal stress.
2 The melting furnace has a constant temperature of 11 The blocks are cut to size and sorted by batch.
1250°C. Production waste is recycled.
3 Molten glass is drawn out of the furnace. 12 FOAMGLAS® slabs are then packaged, labelled
4 Control room for monitoring the production. and palletized.
5 The glass is drawn off and falls onto the conveyor 13 Finished FOAMGLAS® products are stored and
band where it cools down before entering the ball mill. prepared for transport.
6 Addition of "carbon black".
7 Ball mill grinds all ingredients into a fine powder Quality assurance
before putting them into stainless steel moulds. Quality is assured through internal and external
8 The filled moulds pass through a cellulating oven monitoring. The product complies with the Declaration
(foaming furnace) with a temperature of 850°C. of Performance. It also bears the CEN Keymark
This is where the material gains its unique cell
structure.
9 Energy recovery of heat.
4 Environmental Product Declaration Pittsburgh Corning Europe NV – FOAMGLAS® F
2.7 Environment and health during Building Products (AgBB scheme). (emissions test as
manufacturing per EN 16516)
During the entire manufacturing process, no other
health protection measures extending beyond the 2.12 Reference service life
legally specified industrial protection measures for Material composition does not alter during use. The
commercial enterprises are needed. Health and safety declaration of the service life (RSL) is 100 years.
management is in accordance with ISO 45001 and FOAMGLAS® products can be used practically
OHSAS 18001. indefinitely when used as designated. FOAMGLAS®
products are impervious to moisture, ants, acids and
Environmental protection during manufacturing: chemicals.
Water/Soil: www.nachhaltigesbauen.de/austausch/nutzungsdauer
Water incurred during manufacturing and plant n-von-bauteilen/
cleaning is treated mechanically in a waste water
treatment system on the plant site and re-used in the
production process. Waste water corresponds with the 2.13 Extraordinary effects
local specifications and the low Al O suspended
2 3
particles contained in the waste water support waste Fire
water cleaning. Unfaced FOAMGLAS® is classified as Euro class A1 in
accordance with EN 13501-1 Class A1 building
Noise: products do not display any hazard potential regarding
The noise emissions into the environment by smoke development, flammability or burning drips.
production equipment fall short of the permissible limit The melting temperature of FOAMGLAS® insulating
values. slabs is above 1000 °C (DIN 4102-17) and the
maximum application limit temperature is approx. 430
The requirements concerning quality management, °C.
environmental management and energy management Faced FOAMGLAS®, in form of faced blocks or boards
are complied with: (ISO 9001, ISO 14001, ISO 50001) consist of core material class A1 with a facing
classified class E in accordance with EN 13501-1
2.8 Product processing/Installation
Recommendations on product processing depend on Fire protection
the respective product and system and are outlined in Name Value
the respective documentation and data sheets Building material class A1
(available at www.foamglas.com). Burning droplets zero
The product does not contain any concentrations of Smoke gas development zero
substances known to be hazardous to health. Dust
incurred during sawing is inert and non-crystalline. Water
Depending on requirements, FOAMGLAS® elements Thanks to its closed-cell structure, exposure to
are applied dry or using mineral or bituminous moisture cannot impair the insulating properties of
adhesives. FOAMGLAS®. Even when exposed to water over long
The insulating slabs are staggered and butt-joined with periods of time (e.g. floods), the insulating material
or without glue. The professional liability associations' remains intact.
rules apply. When applying the products under review,
conventional industrial protection measures must be Mechanical destruction
observed in accordance with information supplied by FOAMGLAS® is extremely resilient in all respects, and
the manufacturer. there is no risk of mechanical destruction if used as
According to the present state of knowledge, hazards designated. It does not represent any environmental
for water, air and soil cannot arise if FOAMGLAS® is hazards thanks to its mineral composition. See
applied as designated. Material Safety Data Sheets (MSDS) for FOAMGLAS®
and natureplus certificate.
2.9 Packaging
Re-usable wooden pallets, PE shrink foil and 2.14 Re-use phase
cardboard elements serve as packaging material. When sorted, the declared products can be re-ground
Packaging material (PE foil and cardboard) is disposed and re-used as additives in the manufacture of
of on the building site. Thermal utilisation takes place. FOAMGLAS® (material recycling). Otherwise sorted
products - even those still bearing adhesive - are
suitable for re-use as filling material for brick
2.10 Condition of use production, civil engineering, road construction or for
Material composition does not alter during use. sound barriers, for example (material recycling). Within
FOAMGLAS® F products can be used practically the re-use of existing surface insulated with
indefinitely when used as designated. They are FOAMGLAS®, the existing layer can be topped with a
impervious to moisture, pests, acids and chemicals. new layer of FOAMGLAS®.
2.11 Environment and health during use 2.15 Disposal
Ingredients: No particular features regarding the Where the recycling options referred to above are not
material composition for the period of use. In practical, foam glass residue incurred on the
accordance with official emission measurements for construction site as well as residue from
indoor air, FOAMGLAS® F is an insulating material deconstruction can be easily deposited without
which does not display VOC (volatile organic preliminary treatment in Class I landfills thanks to their
compounds) or carcinogenic emissions after 3 and 28 non-leaching mineral components. Packaging can be
days (see section 7.2) according to the German utilised thermally. The waste code number as per the
Committee for the Health-Related Evaluation of
5 Environmental Product Declaration Pittsburgh Corning Europe NV – FOAMGLAS® F
List of Wastes Ordinance (AVV/EWC_Eu waste code)
for FOAMGLAS® (uncontaminated) is 17 06 04. In 2.16 Further information
combination with bituminous waterproofing substances Further information on FOAMGLAS® insulating
and adhesive, waste code number 17 09 04 is for materials are available online on the manufacturer's
unsorted waste. website: www.foamglas.com.
3. LCA: Calculation rules
3.1 Declared Unit the LCA. This recycled glass is regarded as a
The Declaration refers to the life cycle of 1kg waste product and is therefore calculated as
FOAMGLAS® F. The gross density of the product input without loads.
is 165 kg/m³ ± 10%  EU region datasets for grid electricity and
thermal energy from natural gas were used
Declared unit
for taking potential credits.
Name Value Unit
 The calorific values (incineration) of
Declared unit 1 kg
packaging material considered are corrugated
Gross density 165 kg/m3
conversion factor [Mass/Declared board: 14 MJ/kg, polyethene-film (PE): 40
1 -
Unit] MJ/kg and wooden pallet: 16 MJ/kg.
 For the calculation of biogenic content, the
biotic carbon dioxide considered is corrugated
board: 1.57 kg CO /kg corrugated board,
3.2 System boundary 2
wooden pallet: 1.36 kg CO /kg wooden pallet.
Type of EPD: Cradle to Grave with options, modules 2
C1-C4, and module D (A1-A3, C, D and additional
modules)
3.4 Cut-off criteria
The LCA addresses the life cycle stage of production, In the assessment, all available data from the
installation, end-of-life (EoL) and potential benefits production process are considered, ie all raw materials
beyond the system boundaries. used, utilized thermal energy, and electric power
consumption using best available LCI datasets. The
The product stage comprises of modules A1 (raw material and energy flow with a share of less than 1%
material supply), A2 (transport) and A3 (production). (based on the total mass of the product) were
The following individual processes were included in the neglected. The sum of the excluded material flows
product stage A1- A3 of production: does not exceed 5% of mass, energy or environmental
 Processes for providing preliminary products relevance. Machinery, plants and infrastructure
and energy required in the manufacturing process were not
considered.
 Transporting the raw materials and
preliminary materials to the plant
3.5 Background data
 The manufacturing process in the plant The software system "GaBi 9" developed by thinkstep
including energy-related expenses, disposal AG - was used to model and assess the life cycle. The
of residual materials and emissions data sets contained in the GaBi database are
 Production of packaging documented in the online GaBi documentation (2020).
These datasets were applied for energy, transport,
preliminary products and auxiliaries. No data records
Module A4 takes into account the transportation of other than GaBi databases were used.
product to the construction site. The treatment of the
packaging materials is assigned to module A5 . The Life Cycle Assessment was carried out for the
Module C1 takes into accounts the de-construction or geographical scope of Belgium (Tessenderlo plant). If
demolition of the product before taking it for no country-specific data sets were available,
treatment/disposal through means of transportation comparable data sets, preferably DE or EU-28 were
(module C2). Module C3 is the waste processing of the used. For the Tessenderlo plant, renewable energy
product before recycling/recovery/reuse. Landfilling mix of European Green 2019 (Belgium region) was
with residual materials is assigned to module C4 . applied. Electricity source was provided along with
Module D accounts for the potential credits resulting valid energy certificates.
from the thermal and electrical energy generated when
burning packaging materials in module A5 (energy 3.6 Data quality
substitution). All background datasets were taken from the GaBi 9
software database. The background data used for the
There are 3 EoL scenarios in the study: Landfill, Reuse LCA was last revised less than 4 years
and Recycling. Module D/2 takes into account potential ago. Pittsburgh Corning Europe NV supplied current
credits for 100% reuse of material and module D/3 primary production data for 2019. This production data
considers potential credits for replacing kaolin in the was examined for plausibility. The corresponding
brick industry. datasets were available in the database for all
preliminary products used. The data quality can be
3.3 Estimates and assumptions regarded as very good.
 In the product system, external cullet or waste
glass is used as a secondary material /
preliminary product within the framework of
6 Environmental Product Declaration Pittsburgh Corning Europe NV – FOAMGLAS® F
3.7 Period under review
The data in this LCA are based on primary data on 3.9 Comparability
production in 2019 supplied by Pittsburgh Corning Basically, a comparison or an evaluation of EPD data
Europe NV. The volumes of raw materials, energy, is only possible if all the data sets to be compared
auxiliaries and consumables used are considered as were created according to EN 15804 and the building
average annual values. context, respectively the product-specific
characteristics of performance, are taken into account.
3.8 Allocation
The FOAMGLAS® products are produced in a separate The background database is used from GaBi
production line, with no co-products, hence no co- software, version 9.5 and Service pack number used is
product allocation rules were applied. 40
4. LCA: Scenarios and additional technical information
Characteristic product properties
Information on biogenic Carbon
The biogenic carbon content quantifies the amount of
biogenic carbon in a construction product leaving the
factory gate.
Information on Biogenic Carbon Content for the
declared unit
Name Value Unit
Biogenic Carbon Content in product 0 kg C
Biogenic Carbon Content in Reuse, recovery and/or recycling potentials (D),
0.014 kg C
accompanying packaging relevant scenario information
Name Value Unit
Thermal utilization of cardboard from
0.005 kg
Technical Information the packaging
All the following technical scenario information is given Thermal utilization of PE Film (plastic)
0.010 kg
for the declared unit (i.e., 1 kg FOAMGLAS® product) from the packaging
Thermal utilization of wooden pallets
0.032 kg
Transport to the building site (A4) from the packaging
Name Value Unit Recycling potential of FOAMGLAS 0.617 kg
Transport distance 350 km
Capacity utilisation (including empty
61 %
runs)
Installation into the building (A5)
Name Value Unit
Output substances following waste
0.005 kg
treatment on site (Paper)
Output substances following waste
0.010 kg
treatment on site (Plastic)
Output substances following waste
0.032 kg
treatment on site (Wood)
Operational energy use (B6) and Operational water
use (B7)
Name Value Unit
Water consumption - m3
Electricity consumption - kWh
Other energy carriers - MJ
Equipment output - kW
End of life (C1 - C4)
There are 3 End-of-Life scenarios considered in the
study,
Scenario 1: Landfill
Scenario 2: Reuse
Scenario 3: Recycle
Name Value Unit
Landfilling 1 kg
Reuse 1 kg
Recycling 0.617 kg
7 Environmental Product Declaration Pittsburgh Corning Europe NV – FOAMGLAS® F
5. LCA: Results
End-of-Life scenarios: 1. Landfill, 2. Reuse, 3. Recycling
C3 / 2 - Waste processing for reuse
C3 / 3 - Waste processing for recycling
C4 / 1 - Landfill
D - Potential benefits for thermal utilization of packaging materials
D / 2- Potential benefits for reuse
D / 3- Potential benefits for recycling
DESCRIPTION OF THE SYSTEM BOUNDARY (X = INCLUDED IN LCA; ND = MODULE OR INDICATOR NOT
DECLARED; MNR = MODULE NOT RELEVANT)
BENEFITS AND
CONSTRUCTI LOADS
PRODUCT STAGE ON PROCESS USE STAGE END OF LIFE STAGE BEYOND THE
STAGE SYSTEM
BOUNDARIES
8 Environmental Product Declaration Pittsburgh Corning Europe NV – FOAMGLAS® F
lairetam
waR
ylppus tropsnarT
gnirutcafunaM
eht
morf
tropsnarT
etis
eht
ot
etag
ylbmessA esU
ecnanetniaM
riapeR
tnemecalpeR tnemhsibrufeR
ygrene
lanoitarepO esu
retaw
lanoitarepO esu
noitcurtsnoc-eD
noitilomed tropsnarT
gnissecorp
etsaW
lasopsiD -esueR -yrevoceR -gnilcyceR laitnetop
A1 A2 A3 A4 A5 B1 B2 B3 B4 B5 B6 B7 C1 C2 C3 C4 D
X X X X X ND ND MNR MNR MNR ND ND X X X X X
RESULTS OF THE LCA - ENVIRONMENTAL IMPACT according to EN 15804+A2: 1 kg FOAMGLAS® F
Core Indicator Unit A1-A3 A4 A5 C1 C2 C3/2 C3/3 C4/1 D D/2 D/3
GWP-total [kg CO2-Eq.] 1.45E+0 2.91E-2 8.99E-2 6.47E-4 2.35E-3 0.00E+0 2.74E-3 1.53E-2 -3.46E-2 -1.45E+0 -2.00E-1
GWP-fossil [kg CO2-Eq.] 1.49E+0 2.76E-2 2.54E-2 6.40E-4 2.23E-3 0.00E+0 2.71E-3 1.52E-2 -3.45E-2 -1.49E+0 -2.00E-1
GWP-biogenic [kg CO2-Eq.] -4.45E-2 1.32E-3 6.45E-2 1.93E-6 1.06E-4 0.00E+0 2.38E-5 4.86E-5 -7.97E-5 4.45E-2 -3.15E-4
GWP-luluc [kg CO2-Eq.] 1.26E-3 2.25E-4 2.05E-6 4.99E-6 1.81E-5 0.00E+0 3.92E-6 4.37E-5 -2.32E-5 -1.26E-3 -4.81E-5
ODP [kg CFC11-Eq.] 5.39E-14 3.33E-18 2.06E-17 7.41E-20 2.68E-19 0.00E+0 5.95E-17 5.62E-17 -3.45E-16 -5.39E-14 -3.65E-16
AP [mol H+-Eq.] 5.27E-3 2.91E-5 1.46E-5 3.09E-6 7.17E-6 0.00E+0 5.97E-6 1.09E-4 -4.72E-5 -5.27E-3 -1.86E-4
EP-freshwater [kg PO4-Eq.] 1.48E-5 8.43E-8 3.26E-9 1.87E-9 6.79E-9 0.00E+0 7.23E-9 2.60E-8 -4.26E-8 -1.48E-5 -7.33E-8
EP-marine [kg N-Eq.] 1.58E-3 8.62E-6 4.40E-6 1.44E-6 3.23E-6 0.00E+0 1.33E-6 2.80E-5 -1.23E-5 -1.58E-3 -6.66E-5
EP-terrestrial [mol N-Eq.] 1.82E-2 1.03E-4 6.79E-5 1.59E-5 3.61E-5 0.00E+0 1.39E-5 3.08E-4 -1.32E-4 -1.82E-2 -7.32E-4
POCP [kg NMVOC-Eq.] 3.77E-3 2.37E-5 1.20E-5 4.03E-6 6.33E-6 0.00E+0 3.64E-6 8.48E-5 -3.55E-5 -3.77E-3 -2.01E-4
ADPE [kg Sb-Eq.] 2.03E-7 1.99E-9 3.01E-10 4.42E-11 1.60E-10 0.00E+0 7.83E-10 1.36E-9 -5.49E-9 -2.03E-7 -1.42E-8
ADPF [MJ] 2.15E+1 3.69E-1 2.60E-2 8.20E-3 2.97E-2 0.00E+0 4.76E-2 1.99E-1 -5.84E-1 -2.15E+1 -3.29E+0
[m³ world-Eq
WDP 1.24E-1 2.48E-4 9.38E-3 5.51E-6 2.00E-5 0.00E+0 5.90E-4 1.59E-3 -3.42E-3 -1.24E-1 -3.71E-3
deprived]
GWP = Global warming potential; ODP = Depletion potential of the stratospheric ozone layer; AP = Acidification potential of land and water; EP =
Caption Eutrophication potential; POCP = Formation potential of tropospheric ozone photochemical oxidants; ADPE = Abiotic depletion potential for non-
fossil resources; ADPF = Abiotic depletion potential for fossil resources; WDP = Water (user) deprivation potential
RESULTS OF THE LCA - INDICATORS TO DESCRIBE RESOURCE USE according to EN 15804+A2: 1 kg
FOAMGLAS® F
Indicator Unit A1-A3 A4 A5 C1 C2 C3/2 C3/3 C4/1 D D/2 D/3
PERE [MJ] 1.25E+1 2.08E-2 5.86E-1 4.61E-4 1.67E-3 0.00E+0 2.11E-2 2.61E-2 -1.22E-1 -1.25E+1 -1.34E-1
PERM [MJ] 5.80E-1 0.00E+0 -5.80E-1 0.00E+0 0.00E+0 0.00E+0 0.00E+0 0.00E+0 0.00E+0 -5.80E-1 0.00E+0
PERT [MJ] 1.31E+1 2.08E-2 6.00E-3 4.61E-4 1.67E-3 0.00E+0 2.11E-2 2.61E-2 -1.22E-1 -1.31E+1 -1.34E-1
PENRE [MJ] 2.11E+1 3.70E-1 4.06E-1 8.21E-3 2.98E-2 0.00E+0 4.76E-2 1.99E-1 -5.84E-1 -2.11E+1 -3.29E+0
PENRM [MJ] 3.80E-1 0.00E+0 -3.80E-1 0.00E+0 0.00E+0 0.00E+0 0.00E+0 0.00E+0 0.00E+0 -3.80E-1 0.00E+0
PENRT [MJ] 2.15E+1 3.70E-1 2.60E-2 8.21E-3 2.98E-2 0.00E+0 4.76E-2 1.99E-1 -5.84E-1 -2.15E+1 -3.29E+0
SM [kg] 3.83E-1 0.00E+0 0.00E+0 0.00E+0 0.00E+0 0.00E+0 0.00E+0 0.00E+0 0.00E+0 0.00E+0 0.00E+0
RSF [MJ] 0.00E+0 0.00E+0 0.00E+0 0.00E+0 0.00E+0 0.00E+0 0.00E+0 0.00E+0 0.00E+0 0.00E+0 0.00E+0
NRSF [MJ] 0.00E+0 0.00E+0 0.00E+0 0.00E+0 0.00E+0 0.00E+0 0.00E+0 0.00E+0 0.00E+0 0.00E+0 0.00E+0
FW [m³] 2.59E-2 2.40E-5 2.22E-4 5.34E-7 1.94E-6 0.00E+0 2.44E-5 5.02E-5 -1.42E-4 -2.59E-2 -1.57E-4
PERE = Use of renewable primary energy excluding renewable primary energy resources used as raw materials; PERM = Use of
renewable primary energy resources used as raw materials; PERT = Total use of renewable primary energy resources; PENRE = Use of
non-renewable primary energy excluding non-renewable primary energy resources used as raw materials; PENRM = Use of non-
Caption
renewable primary energy resources used as raw materials; PENRT = Total use of non-renewable primary energy resources; SM = Use
of secondary material; RSF = Use of renewable secondary fuels; NRSF = Use of non-renewable secondary fuels; FW = Use of net fresh
water
RESULTS OF THE LCA – WASTE CATEGORIES AND OUTPUT FLOWS according to EN 15804+A2:
1 kg FOAMGLAS® F
Indicator Unit A1-A3 A4 A5 C1 C2 C3/2 C3/3 C4/1 D D/2 D/3
HWD [kg] 6.65E-8 1.72E-8 5.49E-11 3.82E-10 1.39E-9 0.00E+0 1.97E-11 3.03E-9 -2.33E-10 -6.65E-8 -2.77E-9
NHWD [kg] 4.05E-2 5.66E-5 3.16E-3 1.26E-6 4.56E-6 0.00E+0 3.37E-5 1.00E+0 -2.64E-4 -4.05E-2 -8.73E-4
RWD [kg] 8.97E-5 4.58E-7 1.25E-6 1.02E-8 3.68E-8 0.00E+0 7.22E-6 2.26E-6 -4.18E-5 -8.97E-5 -4.40E-5
CRU [kg] 0.00E+0 0.00E+0 0.00E+0 0.00E+0 0.00E+0 1.00E+0 0.00E+0 0.00E+0 0.00E+0 0.00E+0 0.00E+0
MFR [kg] 0.00E+0 0.00E+0 0.00E+0 0.00E+0 0.00E+0 0.00E+0 6.17E-1 0.00E+0 0.00E+0 0.00E+0 0.00E+0
MER [kg] 0.00E+0 0.00E+0 4.66E-2 0.00E+0 0.00E+0 0.00E+0 0.00E+0 0.00E+0 0.00E+0 0.00E+0 0.00E+0
EEE [MJ] 0.00E+0 0.00E+0 1.40E-1 0.00E+0 0.00E+0 0.00E+0 0.00E+0 0.00E+0 0.00E+0 0.00E+0 0.00E+0
EET [MJ] 0.00E+0 0.00E+0 2.74E-1 0.00E+0 0.00E+0 0.00E+0 0.00E+0 0.00E+0 0.00E+0 0.00E+0 0.00E+0
HWD = Hazardous waste disposed; NHWD = Non-hazardous waste disposed; RWD = Radioactive waste disposed; CRU = Components
Caption for re-use; MFR = Materials for recycling; MER = Materials for energy recovery; EEE = Exported electrical energy; EEE = Exported
thermal energy
RESULTS OF THE LCA – additional impact categories according to EN 15804+A2-optional:
1 kg FOAMGLAS® F
Indicator Unit A1-A3 A4 A5 C1 C2 C3/2 C3/3 C4/1 D D/2 D/3
[Disease
PM 5.69E-8 1.71E-10 1.08E-10 3.47E-11 3.92E-11 0.00E+0 5.01E-11 1.35E-9 -4.01E-10 -5.69E-8 -9.95E-9
Incidence]
[kBq U235-
IR 1.28E-2 6.62E-5 1.69E-4 1.47E-6 5.33E-6 0.00E+0 1.18E-3 2.32E-4 -6.85E-3 -1.28E-2 -7.19E-3
Eq.]
ETP-fw [CTUe] 4.69E+1 2.61E-1 1.07E-2 5.80E-3 2.10E-2 0.00E+0 2.03E-2 1.14E-1 -1.21E-1 -4.69E+1 -1.81E-1
HTP-c [CTUh] 5.75E-10 5.47E-12 7.84E-13 1.21E-13 4.40E-13 0.00E+0 5.62E-13 1.68E-11 -5.40E-12 -5.75E-10 -2.46E-11
HTP-nc [CTUh] 2.19E-8 2.83E-10 5.21E-11 7.28E-12 2.58E-11 0.00E+0 2.07E-11 1.86E-9 -2.01E-10 -2.19E-8 -9.43E-10
SQP [-] 2.80E+1 1.30E-1 7.45E-3 2.88E-3 1.04E-2 0.00E+0 1.51E-2 4.15E-2 -8.80E-2 -2.80E+1 -1.07E-1
PM = Potential incidence of disease due to PM emissions; IR = Potential Human exposure efficiency relative to U235; ETP-fw = Potential
Caption comparative Toxic Unit for ecosystems; HTP-c = Potential comparative Toxic Unit for humans (cancerogenic); HTP-nc = Potential
comparative Toxic Unit for humans (not cancerogenic); SQP = Potential soil quality index
The transportation distance to waste processing system (module C2) is considered as 30 km. Specifically, for
scenario 3, i.e. recycling, the transportation distance to the brick industry is 100 km, hence multiply the results in
module C2 by 3.33 (i.e.,100/30) to get the result for 100 km.
The environmental impacts of the coated product are to be assessed with the help of a markup factor in the
amount of 0.8% for Global Warming Potential and for all LCA results, the maximum deviation is 5.44%.
Disclaimer 1 - for the indicator IRPT This impact category deals mainly with the eventual impact of low dose
ionizing radiation on human health of the nuclear fuel cycle. It does not consider effects due to possible nuclear
accidents, occupational exposure nor due to radioactive waste disposal in underground facilities. Potential
ionizing radiation from the soil, from radon and some construction materials is also not measured by this indicator.
Disclaimer 2 - The results of environmental impact indicators ADPE, ADPF, WDP, ETP-fw, HTP-c, HTP-nc, SQP
shall be used with care as the uncertainties on these results are high or as there is limited experience with the
indicator.
6. LCA: Interpretation
The contributions from module A1 (raw materials) and Photochemical ozone formation, net freshwater use;
A3 (energy) dominate in climate change impact. The around 82% contribution in Acidification potential and
modules A4, A5, C1, C2, C3 and C4 contributes less. around 50% contribution in Resource use (energy
The credits i.e. module D results from the incineration carriers) and Total use of renewable and non-
of packaging materials. Module D/2 credit is highest as renewable primary energy resources. The other
the 100% manufacturing impacts of the product are relevant contributor is Feldspar contributing around
taken as a credit for its 100% reuse. 30% in Resource use (energy carriers) and Total use
of renewable and non-renewable primary energy
The significant contributor (> 50%) and relevant resources. 72% of Resource use (mineral and metals)
contributor (25% - 50%) among all the raw materials is contributed by Manganese dioxide as the use of
for most of the impact categories is Sodium carbonate, manganese ore for its production leads to depletion of
with around 60% contribution in Climate change, 70%- mineral and metal resource.
77% contribution in Eutrophication of freshwater,
7. Requisite evidence
7.1 Bio-persistence Engineering, Czech Republic).
FOAMGLAS® products do not contain fibres and also
biocides. 7.3 Leaching
The ELUAT-tests on FOAMGLAS® products according
7.2 Radioactivity the ICP-MS tests method ISO 17294-2 result below
The radon diffusion coefficient FOAMGLAS® products limits (test report Indikator 2017-382). The AOX/EOX
is less than 10-11 (testreport RAD 592 conducted at halogen (ISO 9562) value is zero (Indikator 2017/380).
LaRUC-Radon Group (Uni Cantabria, Spain) –
RiSE/SP Technical Research Institute of Sweden 7.4 Formaldehyde and VOC emissions
Prague Technical University (Faculty of Civil tested according EN 16516, the formaldehyde & VOC
9 Environmental Product Declaration Pittsburgh Corning Europe NV – FOAMGLAS® F
indoor emissions results for FOAMGLAS® products VOC without NIK <5 μg/m3
(Bremer Umwelt H3989; Labo Excell 192-17367; VITO Carcinogenic Substances <1 μg/m3
SERVACO ML02001-28R): Formaldehyde <1 μg/m3
AgBB overview of results (3 days [µg/m³])
Name Value Unit
TVOC (C6 - C16) <5 μg/m3
Sum SVOC (C16 - C22) <5 μg/m3
AgBB overview of results (28 days [µg/m³]) R (dimensionless) 0
Name Value Unit VOC without NIK <5 μg/m3
TVOC (C6 - C16) <5 μg/m3
Carcinogenic Substances <1 μg/m3
Sum SVOC (C16 - C22) <5 μg/m3
Formaldehyde <1 μg/m3
R (dimensionless) 0
8. References
STANDARDS EN ISO 45001:2018, Occupational Health and Safety
Assessment Series (OHSAS) 18001:2007
DIN 4102-17, Fire behaviour of building materials and
building components - Part 17: Melting point of mineral EN ISO 50001:2018, Energy management systems -
wool insulating materials - Terms and definitions, Requirements with guidance for use
requirements and test
OHSAS 18001:2007, Occupational Health - and Safety
EN ISO 9001:2015, Quality management systems – Assessment Series
Requirements
Product Category Rules, Part B: Guidelines for
EN ISO 9562:2004, Water quality - Determination of building-related products and services, Part B:
adsorbable organically bound halogens (AOX) Requirements to be met by the EPD for PCR Mineral
Insulating Materials, Institut Bauen und Umwelt eV,
EN 13167:2015, Thermal insulation products for www.bau-umwelt.com, 2018, version 1.1
buildings - Factory made cellular glass (CG) products
Product Category Rules for Construction Products,
EN 13501-1:2019, Fire classification of construction Part A: Calculation rules for the life cycle assessment
products and building elements - Part 1: Classification and requirements on the background Report according
using data from reaction to fire tests to EN 15804+A2:2019, 2020, version 1.0
EN ISO 14001:2015, Environmental management CERTIFICATES
systems - Requirements with guidance for use
CEN Keymark Certificate n°001-BK-516-001; ATG
EN ISO 14025:2011-10, Environmental labels and H539; KOMO-CTG100-9; SIA CH672-13; ACERMI16-
declarations - Type III environmental declarations - 023-1179;
Principles and procedures (ISO 14025:2006)
Natureplus n°Zt-PCE-0406-1101-101
EN ISO 14040:2009-11, Environmental management -
Life cycle assessment - Principles and framework Green Energy Certificate (Klasterec): KLA-
(ISO 14040:2006) renewable energy, Slovak Power Plants, Pittsburgh
Corning CR
EN ISO 14044:2018-05, Environmental management -
Life cycle assessment - Requirements and guidelines Green Energy Certificate (Tessenderlo): Bron
(ISO 14044:2006 + Amd 1:2017) hernieuwbare energie 2019, Pittsburgh Corning
Europe, Luminus Business Team
EN 14305:2013, Thermal insulation for building
equipment and industrial installations - Factory made MSDS: Material Safety Data Sheets (MSDS) for
cellular glass (CG) products FOAMGLAS®
EN 15804:2020-03, Sustainability of construction FURTHER REFERENCES
works - Environmental Product Declarations - Core
rules for the product category of construction products AgBB: Ausschuss zur gesundheitlichen Bewertung
(EN 15804:2012+A2:2019) von Bauprodukten (2018). Committee for Health-
related Evaluation of Building Products. Requirements
EN 16516:2017, Construction products: Assessment of for the Indoor Air Quality in Buildings: Health-related
release of dangerous substances. Determination of Evaluation Procedure for Emissions of Volatile Organic
emissions into indoor air Compounds (VVOC, VOC and SVOC) from
Building Products
EN ISO 17294-2:2016, Water quality - Application of
inductively coupled plasma mass spectrometry (ICP- AVV/EWC: Abfallverzeichnis-Verordnung
MS) - Part 2: Determination of selected elements (AVV)/European Waste Catalogue (EWC)
including uranium isotopes
10 Environmental Product Declaration Pittsburgh Corning Europe NV – FOAMGLAS® F
Construction Products Regulation (CPR): the Institut Bauen und Umwelt eV Version 1., Berlin:
Regulation (EU) No 305/2011 Of the European Institut Bauen und Umwelt eV, 2016.
Parliament and of the Council of 9 March 2011 laying www.ibu-epd.com
down harmonised conditions for the marketing of
construction products and repealing Council Directive TEST REPORTS
89/106/EEC
Formaldehyde and VOC emissions
ECHA candidate list
Candidate List of substances of very high concern for Testing the product emissions accordance with the
Authorisation AgBB/DIBt method.
http://echa.europa.eu/web/guest/candidate-list-table Tested according DIN EN 16516, the formaldehyde &
(10.02.2021) VOC indoor emissions (Bremer Umwelt H3989; Labo
Excell 192-17367; VITO SERVACO ML02001-28R):
ETA: European Technical Assessment (ETA) 17/0903
Leaching / ELUAT test EMPA, Eidgenössische
ETA: European Technical Assessment (ETA) Materialprüfungs und Forschungsanstalt EMPA. Test
20/0221:2020 Cellular glass boards as load bearing report FOAMGLAS® according the ICP-MS tests
layer and thermal insulation outside the waterproofing method EN ISO 17294-2 (test report Indikator 2017-
382). The AOX/EOX halogen (EN ISO 9562)
EWC: Commission Decision of 18 December 2014 Indikator 2017/380.
amending Decision 2000/532/EC on the list of waste
pursuant to Directive 2008/98/EC of the European Test Report Radioactivity
Parliament and of the Council (RAD 592 conducted at LaRUC-Radon Group (Uni
Cantabria, Spain) – RiSE/SP Technical Research
GaBi 9 2020: Dataset documentation for the software Institute of Sweden Prague Technical University
system and databases, LBP, University of Stuttgart (Faculty of Civil Engineering, Czech Republic).
and Sphera, Leinfelden-Echterdingen, 2020
(http://documentation.gabi-software.com/)
IBU 2016, Institut Bauen und Umwelt eV: General
Program Instructions for the Preparation of EPDs at
11 Environmental Product Declaration Pittsburgh Corning Europe NV – FOAMGLAS® F
Publisher
Institut Bauen und Umwelt e.V. Tel +49 (0)30 3087748- 0
Panoramastr. 1 Fax +49 (0)30 3087748- 29
10178 Berlin Mail info@ibu-epd.com
Germany Web www.ibu-epd.com
Programme holder
Institut Bauen und Umwelt e.V. Tel +49 (0)30 - 3087748- 0
Panoramastr 1 Fax +49 (0)30 – 3087748 - 29
10178 Berlin Mail info@ibu-epd.com
Germany Web www.ibu-epd.com
Author of the Life Cycle
Assessment Tel +49 711 341817-0
Sphera Solutions GmbH Fax +49 711 341817-25
Hauptstraße 111- 113 Mail info@sphera.com
70771 Leinfelden-Echterdingen Web www.sphera.com
Germany
Owner of the Declaration
Pittsburgh Corning Europe NV Tel +32 (0) 13 661721
Albertkade 1 Fax +32 (0) 13 667854
3980 Tessenderlo Mail info@foamglas.dcom
Belgium Web www.foamglas.com
