ENVIRONMENTAL PRODUCT DECLARATION
as per ISO 14025 and EN 15804+A2
Owner of the Declaration Pittsburgh Corning Europe NV
Programme holder Institut Bauen und Umwelt e.V. (IBU)
Publisher Institut Bauen und Umwelt e.V. (IBU)
Declaration number EPD-PCE-20200299-IBB1-EN
Issue date 15.03.2021
Valid to 14.03.2026
FOAMGLAS® T4+
Pittsburgh Corning Europe NV
www.ibu-epd.com | https://epd-online.com
Umwelt Produktdeklaration Name des Herstellers – Name des Produkts
1. General Information
Pittsburgh Corning Europe NV FOAMGLAS® T4+
Programme holder Owner of the declaration
IBU – Institut Bauen und Umwelt e.V. Pittsburgh Corning Europe NV
Panoramastr. 1 Albertkade 1
10178 Berlin B-3980 Tessenderlo
Germany Belgium
Declaration number Declared product / declared unit
EPD-PCE-20200299-IBB1-EN FOAMGLAS® T4+ / declared unit 1 kg uncoated
cellular glass insulation material
This declaration is based on the product Scope:
category rules: This document refers to the production of 1 kg
Mineral insulating materials, 12.2018 uncoated "FOAMGLAS® T4+" cellular glass
(PCR checked and approved by the SVR) manufactured in Belgium at the Tessenderlo
and in Czech Republic at the Klasterec production
facilities of Pittsburgh Corning Europe NV. The
Issue date
reference year of production is 2019.
15.03.2021
The environmental impacts of the coated product
"FOAMGLAS® T4+ in boards & blocks " are to be
Valid to assessed with the help of a markup factor in the
14.03.2026 amount of 0.8% for Global Warming Potential.
Besides FOAMGLAS® T4+, exclusively for building
equipment and industrial applications
FOAMGLAS® ONE has the same environmental
impacts as FOAMGLAS® T4+.
The owner of the declaration shall be liable for the
underlying information and evidence; the IBU shall not
be liable with respect to manufacturer information, life
cycle assessment data and evidences.
The EPD was created according to the specifications
of EN 15804+A2. In the following, the standard will be
simplified as EN 15804.
Verification
The standard EN 15804 serves as the core PCR
Independent verification of the declaration and data
according to ISO 14025:2010
Dipl. Ing. Hans Peters internally x externally
(chairman of Institut Bauen und Umwelt e.V.)
Dr. Alexander Röder Matthias Klingler
(Managing Director Institut Bauen und Umwelt e.V.)) (Independent verifier)
2. Product
2.1 Product description/Product definition mm.
FOAMGLAS® T4+ is an insulation product for
buildings made of cellular glass. It is applied to the For the placing on the market of the product
desired dimensions in the form of slabs, panels, or FOAMGLAS® T4+ in the European Union/European
other specific elements. The FOAMGLAS® T4+ is in Free Trade Association (EU/EFTA) (with the exception
general unfaced as a slab. Further processing to of Switzerland) Construction Products Regulation
fabricated ware is possible (eg PSG, PSH, PSQ,…). In (CPR) applies. The product declaration of performance
some cases, depending on the end-use, the slabs can (DOP) is taking into consideration EN 13167:2015
be faced with bitumen on the top with a PE-foil (e.g. Thermal insulation products for buildings – Factory
READY, BOARDS) or a white mineral liner made cellular glass (CG) products – Specification but
(ROOFBLOCK, ROOF BOARDS). Also, on the bottom, also EN14305:2013 Thermal insulation for building
the white mineral liner can be applied (cf. BOARDS). equipment and industrial installations - Factory made
cellular glass (CG) products – Specification.
The product is declared with a density of 110 kg/m³
(±15%) and is supplied in thicknesses of 40 mm to 200 In addition to the common applications, especially for
loadbearing constructions and perimeter insulation, the
2 Environmental Product Declaration Pittsburgh Corning Europe NV – FOAMGLAS® T4+
product also complies with the characteristics declared
in European Technical Assessment (ETA) 17/0903: 2.4 Delivery status
2017 Cellular glass boards as load bearing layer and FOAMGLAS® T4+ are available in the following
thermal insulation outside the waterproofing and the thicknesses: from 40 to 200 mm
CE-marking. FOAMGLAS® T4+ are available in the following
dimensions:
For the application and use the respective national - Slabs & Blocks: 600x450mm; 300x450mm
provisions apply. - Boards: 1200x600mm
Other dimensions are available on request.
2.2 Application
FOAMGLAS® T4+ products are used for roof, facades,
interior, in contact with the ground, or specific 2.5 Base materials/Ancillary materials
insulation. FOAMGLAS® T4+ is also used for building The main constituents of the product or its
equipment & industrial installations, for which components are:
FOAMGLAS® ONE is an equivalent product. - Sand 15%
- Feldspar 20%
2.3 Technical Data - Recycled content (glass/scrap) 50% to 60%
The technical specifications of FOAMGLAS® T4+ - Others 5% to 15%
within the scope of this EPD and within the CE marking
is according to EN 13167, EN 14305 and ETA. 1) This product/article/at least one partial article
contains substances listed in the ECHA candidate
In addition to the EN13167 declared values, the list (date: 19.01.2021) exceeding 0.1 percentage by
characteristics declared for service temperature (- mass: no
265°C – 430°C), thermal conductivity ranges &
chloride content are in line with EN 14305. The same 2) This product/article/at least one partial article
for the ETA declared values on the mechanical contains other CMR substances in categories 1A or 1B
properities. Performance data of the product in which are not on the candidate list, exceeding 0.1
accordance with the declaration of performance with percentage by mass: no
respect to its essential characteristics according to EN
13167. 3) Biocide products were added to this construction
product or it has been treated with biocide products
Voluntary data: CEN KEYMARK certificate n°001-BK- (this then concerns a treated product as defined by the
516-001; ATG H539; KOMO-CTG100-9; SIA CH672- (EU) Ordinance on Biocide Products No.
13; ACERMI16-023-1179; Natureplus n°Zt-PCE-0406- 528/2012): no
1101-101
2.6 Manufacture
Technical data according EN 13167 The product is made following the protocol of the
Name Value Unit company. All glass constituents (recycled glass, sand,
Thermal conductivity λD 0.041 W/(mK) sodium carbonate, feldspar, sodium sulfate, sodium
Water vapour diffusion resistance ∞ nitrate, iron oxide, and FOAMGLAS®-scrap) are melted
-
factor µ = ∞ (infinite being > 40000) (infinite) (at ca. 1250°C) in the furnace and drawn into the
Gross density 110 kg/m3 shape of a thin-walled tube to enable efficient grinding.
Compressive strength 0.6 N/mm2 Melted glass from the melter furnace is put in grinders
Reaction to fire Class A1 to produce fine glass powder. In the grinding process,
DS70/90 additives are added so that afterwards, glass foaming
Dimensional stability at 70°C/95%RH (≤0.5mm processes can be envisaged. In the foaming furnace,
) cellular glass blocks are made in moulds by heating
Water absorption (short/long) ≤ 0.5 kg/m² (sintering towards ca 850°C) the glass powder after the
grinding process. After the foaming process, the
Point load PL ≤ 1.5 mm
annealing process starts by moving the foamed blocks
BS ≥
Bending Strength kPa on the lehr where they cool according to a precisely
450
determined curve. The cooled blocks are cut into
CC(1.5/1
Compressive creep (long behaviour) kPa rectangular blocks and if necessary, ground or cut to
/50)225
thinner sizes. The produced material is released,
labelled, marked, and packed for commercialisation
and various end-use applications (floor, roof, wall,
façade and other construction elements).
3 Environmental Product Declaration Pittsburgh Corning Europe NV – FOAMGLAS® T4+
1 Mixing and batching of the raw materials: Recycled 10 The FOAMGLAS® blocks pass through an
glass, feldspar, sodium carbonate, iron oxide, annealing oven to allow carefully controlled cooling
manganese oxide, sodium sulphate, sodium nitrate. without thermal stress.
2 The melting furnace has a constant temperature of 11 The blocks are cut to size and sorted by batch.
1250°C. Production waste is recycled.
3 Molten glass is drawn out of the furnace. 12 FOAMGLAS® slabs are then packaged, labelled
4 Control room for monitoring the production. and palletized.
5 The glass is drawn off and falls onto the conveyor 13 Finished FOAMGLAS® products are stored and
band where it cools down before entering the ball mill. prepared for transport.
6 Addition of "carbon black".
7 Ball mill grinds all ingredients into a fine powder Quality assurance
before putting them into stainless steel moulds. Quality is assured through internal and external
8 The filled moulds pass through a cellulating oven monitoring. The product complies with the Declaration
(foaming furnace) with a temperature of 850°C. of Performance. It also bears the CEN Keymark
This is where the material gains its unique cell
structure.
9 Energy recovery of heat.
4 Environmental Product Declaration Pittsburgh Corning Europe NV – FOAMGLAS® T4+
2.7 Environment and health during Committee for the Health-Related Evaluation of
manufacturing Building Products (AgBB scheme). (emissions test as
During the entire manufacturing process, no other per EN 16516)
health protection measures extending beyond the
legally specified industrial protection measures for 2.12 Reference service life
commercial enterprises are needed. Health and safety Material composition does not alter during use. The
management is in accordance with EN ISO 45001 and declaration of the service life (RSL) is 100 years.
OHSAS 18001 FOAMGLAS® products can be used practically
indefinitely when used as designated. FOAMGLAS®
Environmental protection during manufacturing: products are impervious to moisture, ants, acids and
Water/Soil: chemicals.
Water incurred during manufacturing and plant www.nachhaltigesbauen.de/austausch/nutzungsdauer
cleaning is treated mechanically in a waste water n-von-bauteilen/
treatment system on the plant site and re-used in the
production process. Waste water corresponds with the
local specifications and the low Al O suspended 2.13 Extraordinary effects
2 3
particles contained in the waste water support waste
water cleaning. Fire
Unfaced FOAMGLAS® is classified as Euro class A1 in
Noise: accordance with EN 13501-1 Class A1 building
The noise emissions into the environment by products do not display any hazard potential regarding
production equipment fall short of the permissible limit smoke development, flammability or burning drips.
values. The melting temperature of FOAMGLAS® insulating
slabs is above 1000 °C (DIN 4102-17) and the
The requirements concerning quality management, maximum application limit temperature is approx. 430
environmental management and energy management °C. Faced FOAMGLAS®, in form of faced blocks or
are complied with: (EN ISO 9001, EN ISO 14001, EN boards, consist of core material class A1 with a facing
ISO 50001) classified class E in accordance with EN 13501-1.
2.8 Product processing/Installation Fire protection
Recommendations on product processing depend on Name Value
the respective product and system and are outlined in Building material class A1
the respective documentation and data sheets Burning droplets zero
(available at www.foamglas.com). Smoke gas development zero
The product does not contain any concentrations of
substances known to be hazardous to health. Dust Water
incurred during sawing is inert and non-crystalline. Thanks to its closed-cell structure, exposure to
Depending on requirements, FOAMGLAS® elements moisture cannot impair the insulating properties of
are applied dry or using mineral or bituminous FOAMGLAS®. Even when exposed to water over long
adhesives. periods of time (e.g. floods), the insulating material
The insulating slabs are staggered and butt-joined with remains intact.
or without glue. The professional liability associations'
rules apply. When applying the products under review, Mechanical destruction
conventional industrial protection measures must be FOAMGLAS® is extremely resilient in all respects, and
observed in accordance with information supplied by there is no risk of mechanical destruction if used as
the manufacturer. designated. It does not represent any environmental
According to the present state of knowledge, hazards hazards thanks to its mineral composition. See
for water, air and soil cannot arise if FOAMGLAS® is Material Safety Data Sheets for FOAMGLAS® and
applied as designated. natureplus certificate.
2.9 Packaging 2.14 Re-use phase
Re-usable wooden pallets, PE shrink foil and When sorted, the declared products can be re-ground
cardboard elements serve as packaging material. and re-used as additives in the manufacture of
Packaging material (PE foil and cardboard) is disposed FOAMGLAS® (material recycling). Otherwise sorted
of on the building site. Thermal utilisation takes place. products - even those still bearing adhesive – are
suitable for re-use as filling material for brick
production, civil engineering, road construction or for
2.10 Condition of use sound barriers, for example (material recycling). Within
Material composition does not alter during use. the re-use of existing surface insulated with
FOAMGLAS® T4+ products can be used practically FOAMGLAS®, the existing layer can be topped with a
indefinitely when used as designated. They are new layer of FOAMGLAS®.
impervious to moisture, pests, acids and chemicals.
2.15 Disposal
2.11 Environment and health during use Where the recycling options referred to above are not
Ingredients: No particular features regarding the practical, foam glass residue incurred on the
material composition for the period of use. In construction site as well as residue from
accordance with official emission measurements for deconstruction can be easily deposited without
indoor air, FOAMGLAS® T4+ is an insulating material preliminary treatment in Class I landfills thanks to their
which does not display VOC (volatile organic non-leaching mineral components. Packaging can be
compounds) or carcinogenic emissions after 3 and 28 utilised thermally. The waste code number as per the
days (see section 7.2) according to the German
5 Environmental Product Declaration Pittsburgh Corning Europe NV – FOAMGLAS® T4+
List of Wastes Ordinance (AVV/EWC) for
FOAMGLAS® (uncontaminated) is 17 06 04. In 2.16 Further information
combination with bituminous waterproofing substances Further information on FOAMGLAS® insulating
and adhesive, waste code number 17 09 04 is for materials is available online on the manufacturer's
unsorted waste. website: www.foamglas.com.
3. LCA: Calculation rules
3.1 Declared Unit  In the product system, external cullet or waste
The Declaration refers to the life cycle of 1kg glass is used as a secondary
FOAMGLAS® T4+. The gross density of the product
material/preliminary product within the
is 110 kg/m³ ± 15%.
framework of the LCA. This recycled glass is
regarded as a waste product and is therefore
Declared unit
Name Value Unit calculated as input without loads.
Declared unit 1 kg  EU region datasets for grid electricity and thermal
Gross density 110 kg/m3 energy from natural gas were used for taking
conversion factor [Mass/Declared 1 - potential credits.
Unit]
 The calorific values (incineration) of packaging
material considered are corrugated board: 14
MJ/kg, polyethene-film (PE): 40 MJ/kg and
3.2 System boundary wooden pallet: 16 MJ/kg.
Type of EPD: Cradle to Grave with options, modules  For the calculation of biogenic content, the biotic
C1-C4, and module D (A1-A3, C, D and additional carbon dioxide considered is corrugated board:
modules)
1.57 kg CO /kg corrugated board, wooden pallet:
2
1.36 kg CO /kg wooden pallet.
The LCA addresses the life cycle stage of production, 2
installation, end-of-life (EoL) and potential benefits
beyond the system boundaries.
3.4 Cut-off criteria
The product stage comprises of modules A1 (raw In the assessment, all available data from the
material supply), A2 (transport) and A3 (production). production process are considered, i.e. all raw
The following individual processes were included in the materials used, utilized thermal energy, and electric
product stage A1- A3 of production: power consumption using best available LCI datasets.
 Processes for providing preliminary products The material and energy flow with a share of less than
and energy 1% (based on the total mass of the product) were
neglected. The sum of the excluded material flows
 Transporting the raw materials and
does not exceed 5% of mass, energy or environmental
preliminary materials to the plant
relevance. Machinery, plants and infrastructure
 The manufacturing process in the plant required in the manufacturing process was not
including energy-related expenses, disposal considered.
of residual materials and emissions
 Production of packaging 3.5 Background data
The software system "GaBi 9 2020" developed by
thinkstep AG - was used to model and assess the life
Module A4 takes into account the transportation of cycle. The data sets contained in the GaBi database
product to the construction site. The treatment of the are documented in the online GaBi documentation
packaging materials is assigned to module A5. Module (2020). These datasets were applied for energy,
C1 takes into accounts the de-construction or transport, preliminary products and auxiliaries. No data
demolition of the product before taking it for treatment / records other than GaBi databases were used.
disposal through means of transportation (module C2).
Module C3 is the waste processing of the product The Life Cycle Assessment was carried out for the
before recycling/recovery/reuse. Landfilling with geographical scope of Belgium (Tessenderlo plant)
residual materials is assigned to module C4. Module D and the Czech Republic (Klasterec plant). If no
accounts for the potential credits resulting from the country-specific data sets were available, comparable
thermal and electrical energy generated when burning data sets, preferably DE or EU-28 were used. For the
packaging materials in module A5 (energy Pittsburgh Corning Europe NV Tessenderlo plant,
substitution). renewable energy mix of European Green 2019 was
applied. For the Klasterec plant, electricity from
There are 3 EoL scenarios in the study: Landfill, Reuse hydropower (Slovakia region) was applied. Electricity
and Recycling. Module D/2 takes into account potential source for both plants was provided along with valid
credits for 100% reuse of material and module D/3 energy certificates.
considers potential credits for replacing kaolin in the
brick industry. 3.6 Data quality
All background datasets were taken from the GaBi 9
3.3 Estimates and assumptions 2020 software database. The background data used
 An average product based on production for the LCA was last revised less than 4 years ago.
volume in Tessenderlo and Klasterec was Pittsburgh Corning Europe NV supplied
calculated.
6 Environmental Product Declaration Pittsburgh Corning Europe NV – FOAMGLAS® T4+
current primary production data for 2019. This 3.8 Allocation
production data was examined for plausibility. The FOAMGLAS® products are produced in a separate
The corresponding datasets were available in the production line, with no co-products, hence no co-
database for all preliminary products used. The data product allocation rules were applied.
quality can be regarded as very good.
3.9 Comparability
3.7 Period under review Basically, a comparison or an evaluation of EPD data
The data in this LCA are based on primary data is only possible if all the data sets to be compared
on production in 2019 supplied by Pittsburgh Corning were created according to EN 15804 and the building
Europe NV. The volumes of raw materials, energy, context, respectively the product-specific
auxiliaries and consumables used are considered as characteristics of performance, are taken into account.
average annual values.
The background database is used from GaBi
software, version 9.5 and Service pack number of the
database used is 40
4. LCA: Scenarios and additional technical information
Characteristic product properties Thermal utilization of PE Film (plastic)
0.016 kg
Information on biogenic Carbon from the packaging
The biogenic carbon content quantifies the amount of Thermal utilization of wooden pallets
0.038 kg
biogenic carbon in a construction product leaving the from the packaging
factory gate. Recycling potential of FOAMGLAS 0.546 kg
Information on Biogenic Carbon Content for
declared unit
Name Value Unit
Biogenic Carbon Content in product 0 kg C
Biogenic Carbon Content in
0.017 kg C
accompanying packaging
All the following technical scenario information is given
for the declared unit (i.e., 1 kg FOAMGLAS® product)
Transport to the building site (A4)
Name Value Unit
Transport distance 350 km
Capacity utilisation (including empty
61 %
runs)
Installation into the building (A5)
Name Value Unit
Output substances following waste
0.007 kg
treatment on site (Paper)
Output substances following waste
0.016 kg
treatment on site (Plastic)
Output substances following waste
0.038 kg
treatment on site (Wood)
End of life (C1 - C4)
There are 3 End-of-Life scenarios considered in the
study,
Scenario 1: Landfill
Scenario 2: Reuse
Scenario 3: Recycle
Name Value Unit
Landfilling 1 kg
Reuse 1 kg
Recycled 0.546 kg
Reuse, recovery and/or recycling potentials (D),
relevant scenario information
Name Value Unit
Thermal utilization of cardboard from
0.007 kg
the packaging
7 Environmental Product Declaration Pittsburgh Corning Europe NV – FOAMGLAS® T4+
5. LCA: Results
End-of-Life scenarios: 1. Landfill, 2. Reuse, 3. Recycling
C3 / 2 - Waste processing for reuse
C3 / 3 - Waste processing for recycling
C4 / 1 - Landfill
D - Potential benefits for thermal utilization of packaging materials
D / 2- Potential benefits for reuse
D / 3- Potential benefits for recycling
DESCRIPTION OF THE SYSTEM BOUNDARY (X = INCLUDED IN LCA; ND = MODULE OR INDICATOR NOT
DECLARED; MNR = MODULE NOT RELEVANT)
BENEFITS AND
CONSTRUCTI LOADS
PRODUCT STAGE ON PROCESS USE STAGE END OF LIFE STAGE BEYOND THE
STAGE SYSTEM
BOUNDARIES
8 Environmental Product Declaration Pittsburgh Corning Europe NV – FOAMGLAS® T4+
lairetam
waR
ylppus tropsnarT
gnirutcafunaM
eht
morf
tropsnarT
etis
eht
ot
etag
ylbmessA esU
ecnanetniaM
riapeR
tnemecalpeR tnemhsibrufeR
ygrene
lanoitarepO esu
retaw
lanoitarepO esu
noitcurtsnoc-eD
noitilomed tropsnarT
gnissecorp
etsaW
lasopsiD -esueR -yrevoceR -gnilcyceR laitnetop
A1 A2 A3 A4 A5 B1 B2 B3 B4 B5 B6 B7 C1 C2 C3 C4 D
X X X X X ND ND MNR MNR MNR ND ND X X X X X
RESULTS OF THE LCA - ENVIRONMENTAL IMPACT according to EN 15804+A2: 1 kg FOAMGLAS® T4+
Core Indicator Unit A1-A3 A4 A5 C1 C2 C3/2 C3/3 C4/1 D D/2 D/3
GWP-total [kg CO2-Eq.] 1.43E+0 2.96E-2 1.21E-1 6.16E-4 2.35E-3 0.00E+0 2.41E-3 1.53E-2 -4.79E-2 -1.43E+0 -1.77E-1
GWP-fossil [kg CO2-Eq.] 1.49E+0 2.80E-2 4.23E-2 6.40E-4 2.23E-3 0.00E+0 2.39E-3 1.52E-2 -4.78E-2 -1.49E+0 -1.77E-1
GWP-biogenic [kg CO2-Eq.] -5.62E-2 1.33E-3 7.88E-2 1.93E-6 1.06E-4 0.00E+0 2.11E-5 4.86E-5 -1.10E-4 5.62E-2 -2.79E-4
GWP-luluc [kg CO2-Eq.] 1.10E-3 2.28E-4 3.16E-6 4.99E-6 1.81E-5 0.00E+0 3.47E-6 4.37E-5 -3.18E-5 -1.10E-3 -4.25E-5
ODP [kg CFC11-Eq.] 8.21E-14 3.38E-18 3.10E-17 7.41E-20 2.68E-19 0.00E+0 5.27E-17 5.62E-17 -4.73E-16 -8.21E-14 -3.23E-16
AP [mol H+-Eq.] 5.08E-3 2.95E-5 2.02E-5 3.09E-6 7.17E-6 0.00E+0 5.28E-6 1.09E-4 -6.51E-5 -5.08E-3 -1.64E-4
EP-freshwater [kg PO4-Eq.] 1.99E-5 8.56E-8 4.92E-9 1.87E-9 6.79E-9 0.00E+0 6.39E-9 2.60E-8 -5.86E-8 -1.99E-5 -6.49E-8
EP-marine [kg N-Eq.] 1.67E-3 8.75E-6 5.94E-6 1.44E-6 3.23E-6 0.00E+0 1.17E-6 2.80E-5 -1.70E-5 -1.67E-3 -5.89E-5
EP-terrestrial [mol N-Eq.] 1.85E-2 1.05E-4 9.34E-5 1.59E-5 3.61E-5 0.00E+0 1.23E-5 3.08E-4 -1.83E-4 -1.85E-2 -6.48E-4
POCP [kg NMVOC-Eq.] 3.93E-3 2.40E-5 1.62E-5 4.03E-6 6.33E-6 0.00E+0 3.22E-6 8.48E-5 -4.91E-5 -3.93E-3 -1.78E-4
ADPE [kg Sb-Eq.] 2.18E-7 2.02E-9 4.48E-10 4.42E-11 1.60E-10 0.00E+0 6.93E-10 1.36E-9 -7.57E-9 -2.18E-7 -1.26E-8
ADPF [MJ] 2.22E+1 3.75E-1 3.72E-2 8.20E-3 2.97E-2 0.00E+0 4.21E-2 1.99E-1 -8.10E-1 -2.22E+1 -2.91E+0
[m³ world-Eq
WDP 1.25E-1 2.52E-4 1.27E-2 5.51E-6 2.00E-5 0.00E+0 5.22E-4 1.59E-3 -4.70E-3 -1.25E-1 -3.28E-3
deprived]
GWP = Global warming potential; ODP = Depletion potential of the stratospheric ozone layer; AP = Acidification potential of land and water; EP =
Caption Eutrophication potential; POCP = Formation potential of tropospheric ozone photochemical oxidants; ADPE = Abiotic depletion potential for non-
fossil resources; ADPF = Abiotic depletion potential for fossil resources; WDP = Water (user) deprivation potential
RESULTS OF THE LCA - INDICATORS TO DESCRIBE RESOURCE USE according to EN 15804+A2: 1 kg
FOAMGLAS® T4+
Indicator Unit A1-A3 A4 A5 C1 C2 C3/2 C3/3 C4/1 D D/2 D/3
PERE [MJ] 1.28E+1 2.11E-2 7.28E-1 4.61E-4 1.67E-3 0.00E+0 1.87E-2 2.61E-2 -1.68E-1 -1.28E+1 -1.18E-1
PERM [MJ] 7.20E-1 0.00E+0 -7.20E-1 0.00E+0 0.00E+0 0.00E+0 0.00E+0 0.00E+0 0.00E+0 -7.20E-1 0.00E+0
PERT [MJ] 1.35E+1 2.11E-2 8.00E-3 4.61E-4 1.67E-3 0.00E+0 1.87E-2 2.61E-2 -1.68E-1 -1.35E+1 -1.18E-1
PENRE [MJ] 2.16E+1 3.75E-1 6.77E-1 8.21E-3 2.98E-2 0.00E+0 4.21E-2 1.99E-1 -8.10E-1 -2.16E+1 -2.91E+0
PENRM [MJ] 6.40E-1 0.00E+0 -6.40E-1 0.00E+0 0.00E+0 0.00E+0 0.00E+0 0.00E+0 0.00E+0 -6.40E-1 0.00E+0
PENRT [MJ] 2.22E+1 3.75E-1 3.70E-2 8.21E-3 2.98E-2 0.00E+0 4.21E-2 1.99E-1 -8.10E-1 -2.22E+1 -2.91E+0
SM [kg] 4.54E-1 0.00E+0 0.00E+0 0.00E+0 0.00E+0 0.00E+0 0.00E+0 0.00E+0 0.00E+0 0.00E+0 0.00E+0
RSF [MJ] 0.00E+0 0.00E+0 0.00E+0 0.00E+0 0.00E+0 0.00E+0 0.00E+0 0.00E+0 0.00E+0 0.00E+0 0.00E+0
NRSF [MJ] 0.00E+0 0.00E+0 0.00E+0 0.00E+0 0.00E+0 0.00E+0 0.00E+0 0.00E+0 0.00E+0 0.00E+0 0.00E+0
FW [m³] 3.13E-2 2.44E-5 2.99E-4 5.34E-7 1.94E-6 0.00E+0 2.16E-5 5.02E-5 -1.95E-4 -3.13E-2 -1.39E-4
PERE = Use of renewable primary energy excluding renewable primary energy resources used as raw materials; PERM = Use of
renewable primary energy resources used as raw materials; PERT = Total use of renewable primary energy resources; PENRE = Use of
non-renewable primary energy excluding non-renewable primary energy resources used as raw materials; PENRM = Use of non-
Caption
renewable primary energy resources used as raw materials; PENRT = Total use of non-renewable primary energy resources; SM = Use
of secondary material; RSF = Use of renewable secondary fuels; NRSF = Use of non-renewable secondary fuels; FW = Use of net fresh
water
RESULTS OF THE LCA – WASTE CATEGORIES AND OUTPUT FLOWS according to EN 15804+A2:
1 kg FOAMGLAS® T4+
Indicator Unit A1-A3 A4 A5 C1 C2 C3/2 C3/3 C4/1 D D/2 D/3
HWD [kg] 6.03E-8 1.75E-8 8.76E-11 3.82E-10 1.39E-9 0.00E+0 1.74E-11 3.03E-9 -3.22E-10 -6.03E-8 -2.45E-9
NHWD [kg] 4.09E-2 5.74E-5 5.08E-3 1.26E-6 4.56E-6 0.00E+0 2.99E-5 1.00E+0 -3.64E-4 -4.09E-2 -7.72E-4
RWD [kg] 9.95E-5 4.64E-7 1.73E-6 1.02E-8 3.68E-8 0.00E+0 6.39E-6 2.26E-6 -5.73E-5 -9.95E-5 -3.90E-5
CRU [kg] 0.00E+0 0.00E+0 0.00E+0 0.00E+0 0.00E+0 1.00E+0 0.00E+0 0.00E+0 0.00E+0 0.00E+0 0.00E+0
MFR [kg] 0.00E+0 0.00E+0 0.00E+0 0.00E+0 0.00E+0 0.00E+0 5.46E-1 0.00E+0 0.00E+0 0.00E+0 0.00E+0
MER [kg] 0.00E+0 0.00E+0 6.18E-2 0.00E+0 0.00E+0 0.00E+0 0.00E+0 0.00E+0 0.00E+0 0.00E+0 0.00E+0
EEE [MJ] 0.00E+0 0.00E+0 1.92E-1 0.00E+0 0.00E+0 0.00E+0 0.00E+0 0.00E+0 0.00E+0 0.00E+0 0.00E+0
EET [MJ] 0.00E+0 0.00E+0 3.83E-1 0.00E+0 0.00E+0 0.00E+0 0.00E+0 0.00E+0 0.00E+0 0.00E+0 0.00E+0
HWD = Hazardous waste disposed; NHWD = Non-hazardous waste disposed; RWD = Radioactive waste disposed; CRU = Components
Caption for re-use; MFR = Materials for recycling; MER = Materials for energy recovery; EEE = Exported electrical energy; EEE = Exported
thermal energy
RESULTS OF THE LCA – additional impact categories according to EN 15804+A2-optional:
1 kg FOAMGLAS® T4+
Indicator Unit A1-A3 A4 A5 C1 C2 C3/2 C3/3 C4/1 D D/2 D/3
[Disease
PM 5.46E-8 1.73E-10 1.59E-10 3.47E-11 3.92E-11 0.00E+0 4.43E-11 1.35E-9 -5.54E-10 -5.46E-8 -8.80E-9
Incidence]
[kBq U235-
IR 1.40E-2 6.71E-5 2.25E-4 1.47E-6 5.33E-6 0.00E+0 1.05E-3 2.32E-4 -9.41E-3 -1.40E-2 -6.36E-3
Eq.]
ETP-fw [CTUe] 4.33E+1 2.65E-1 1.52E-2 5.80E-3 2.10E-2 0.00E+0 1.80E-2 1.14E-1 -1.66E-1 -4.33E+1 -1.60E-1
HTP-c [CTUh] 6.93E-10 5.55E-12 1.13E-12 1.21E-13 4.40E-13 0.00E+0 4.97E-13 1.68E-11 -7.47E-12 -6.93E-10 -2.18E-11
HTP-nc [CTUh] 2.78E-8 2.87E-10 8.11E-11 7.28E-12 2.58E-11 0.00E+0 1.83E-11 1.86E-9 -2.78E-10 -2.78E-8 -8.34E-10
SQP [-] 2.50E+1 1.31E-1 1.07E-2 2.88E-3 1.04E-2 0.00E+0 1.34E-2 4.15E-2 -1.21E-1 -2.50E+1 -9.43E-2
PM = Potential incidence of disease due to PM emissions; IR = Potential Human exposure efficiency relative to U235; ETP-fw = Potential
Caption comparative Toxic Unit for ecosystems; HTP-c = Potential comparative Toxic Unit for humans (cancerogenic); HTP-nc = Potential
comparative Toxic Unit for humans (not cancerogenic); SQP = Potential soil quality index
The transportation distance to waste processing system (module C2) is considered as 30 km. Specifically, for
scenario 3, ie recycling, the transportation distance to the brick industry is 100 km, hence multiply the results in
module C2 by 3.33 (i.e., 100/30) to get the result for 100 km.
The environmental impacts of the coated product are to be assessed with the help of a markup factor in the
amount of 0.8% for Global Warming Potential and for all LCA results, the maximum deviation is 5.44%.
Disclaimer 1 - For the indicator IRPT This impact category deals mainly with the eventual impact of low dose
ionizing radiation on human health of the nuclear fuel cycle. It does not consider effects due to possible nuclear
accidents, occupational exposure nor due to radioactive waste disposal in underground facilities. Potential
ionizing radiation from the soil, from radon and some construction materials is also not measured by this indicator.
Disclaimer 2 - The results of environmental impact indicators ADPE, ADPF, WDP, ETP-fw, HTP-c, HTP-nc, SQP
shall be used with care as the uncertainties on these results are high or as there is limited experience with the
indicator.
6. LCA: Interpretation
The contributions from module A1 (raw materials) and potential, Photochemical ozone formation and Net
A3 (energy) dominate in climate change impact. The fresh water use; around 60% impact in Climate change
modules A4, A5, C1, C2, C3 and C4 contributes less. and Eutrophication freshwater; and around 40%
The credits in this study i.e. module D result from the contribution in Ozone depletion, Resource use (energy
incineration of packaging materials. Module D/2 credit carriers) and Total use of renewable and non-
is highest as the 100% manufacturing impacts of the renewable primary energy resources. Feldspar is the
product are taken as a credit for its 100% reuse. second major contributor with around 30% contribution
in Climate change, Resource use (energy carriers) and
The significant contributor (> 50%) and the relevant Total use of renewable and non-renewable primary
contributor (25% - 50%) among all the raw materials in energy resources. Mangenese dioxide contributes 68%
most of the impact categories is Sodium carbonate, in Resource use (mineral and metals).
with more than 75% contribution in Acidification
7. Requisite evidence
7.1 Bio-persistence 7.3 Leaching
FOAMGLAS® products do not contain fibres and also The ELUAT-tests on FOAMGLAS® products according
biocides. the ICP-MS tests method ISO 17294-2 result below
limits (test report No 2017-382 conducted by Indikator
7.2 Radioactivity laboratory ). The AOX/EOX halogen (ISO 9562) value
The radon diffusion coefficient FOAMGLAS® products is zero (test report No 2017-380 Indikator laboratory).
is less than 10-11 testreport No RAD 592 conducted at
LaRUC Uni Cantabria of Spain – RiSE/SP Technical 7.4 Formaldehyde and VOC emissions
Research Institute of Sweden, Prague Technical tested according EN 16516, the formaldehyde & VOC
University of Czech Republic. indoor emissions results for FOAMGLAS® products
(Laboratory Bremer Umweltinstitut No H3989 at
9 Environmental Product Declaration Pittsburgh Corning Europe NV – FOAMGLAS® T4+
Bremen, Germany; Laboratoire Excell at Mérignac in Carcinogenic Substances <1 μg/m3
France, No 192-17367; VITO SERVACO at Mol, Formaldehyde <1 μg/m3
Belgium No ML02001-28R):
The following AgBB evaluation test results for
Formaldehyde and VOC emissions refer to section 7.4
AgBB overview of results (3 days [µg/m³])
The following AgBB evaluation test results for Name Value Unit
Formaldehyde and VOC emissions refer to section 7.4 TVOC (C6 - C16) <5 μg/m3
Sum SVOC (C16 - C22) <5 μg/m3
AgBB overview of results (28 days [µg/m³]) R (dimensionless) 0
Name Value Unit VOC without NIK <5 μg/m3
TVOC (C6 - C16) <5 μg/m3
Carcinogenic Substances <1 μg/m3
Sum SVOC (C16 - C22) <5 μg/m3
Formaldehyde <1 μg/m3
R (dimensionless) 0
VOC without NIK <5 μg/m3
8. References
STANDARDS EN 15804
EN 15804:2020-03 Sustainability of construction works
DIN 4102-17 - Environmental Product Declarations - Core rules for
DIN 4102-17:2017-12 Fire behaviour of building the product category of construction products
materials and building components - Part 17: Melting (EN 15804:2012+A2:2019)
point of mineral wool insulating materials - Terms and
definitions, requirements and test EN 16516
EN 16516:2020-10 Construction products: Assessment
EN ISO 9001 of release of dangerous substances. Determination of
EN ISO 9001:2015-11 Quality management systems – emissions into indoor air
Requirements
EN ISO 17294-2
EN ISO 9562 EN ISO 17294-2:2017-01 Water quality - Application of
EN ISO 9562:2005-02 Water quality - Determination of inductively coupled plasma mass spectrometry (ICP-
adsorbable organically bound halogens (AOX) MS) - Part 2: Determination of selected elements
including uranium isotopes
EN 13167
EN 13167:2012+A1:2015/prA2:2018 Thermal EN ISO 45001
insulation products for buildings - Factory made EN ISO 45001:2018-06 Occupational Health and
cellular glass (CG) products Safety Assessment Series (OHSAS) 18001:2007
EN 13501-1 EN ISO 50001
EN 13501-1:2019-05, Fire classification of construction EN ISO 50001:2018-12 Energy management systems
products and building elements - Part 1: Classification - Requirements with guidance for use
using data from reaction to fire tests
Product Category Rules, Part B: Guidelines for
EN ISO 14001 building-related products and services, Part B:
EN ISO 14001:2015-11 Environmental management Requirements to be met by the EPD for PCR Mineral
systems - Requirements with guidance for use Insulating Materials, Institut Bauen und Umwelt eV,
www.bau-umwelt.com, 2018, version 1.1
EN ISO 14025
EN ISO 14025:2011-10 Environmental labels and Product Category Rules for Construction Products,
declarations - Type III environmental declarations - Part A: Calculation rules for the life cycle assessment
Principles and procedures (ISO 14025:2006) and requirements on the background Report according
to EN 15804+A2:2019, 2020, version 1.0
EN ISO 14040
EN ISO 14040:2021-02 Environmental management - CERTIFICATES
Life cycle assessment - Principles and framework
(ISO 14040:2006) CEN Keymark Certificate n°001-BK-516-001; ATG
H539; KOMO-CTG100-9; SIA CH672-13; ACERMI16-
EN ISO 14044 023-1179;
EN ISO 14044:2021-02 Environmental management -
Life cycle assessment - Requirements and guidelines ECHA candidate list
(ISO 14044:2006 + Amd 1:2017) Candidate List substances in articles
(date: 19.01.2021)
EN 14305
EN 14305:2016-03 Thermal insulation for building Natureplus n°Zt-PCE-0406-1101-101
equipment and industrial installations - Factory made
cellular glass (CG) products Green Energy Certificate (Klasterec)
KLA-renewable energy, Slovak Power Plants,
Pittsburgh Corning CR
10 Environmental Product Declaration Pittsburgh Corning Europe NV – FOAMGLAS® T4+
down harmonised conditions for the marketing of
Green Energy Certificate (Tessenderlo) construction products and repealing Council Directive
Bron hernieuwbare energie 2019, Pittsburgh Corning 89/106/EEC
Europe, Luminus Business Team
ETA
FURTHER REFERENCES European Technical Assessment (ETA) 17/0903:2020
Cellular glass boards as load bearing layer and
AgBB thermal insulation outside the waterproofing
Ausschuss zur gesundheitlichen Bewertung
von Bauprodukten (2018). Committee for Health- GaBi 9 2020
related Evaluation of Building Products. Requirements Dataset documentation for the software system and
for the Indoor Air Quality in Buildings: Health-related databases, LBP, University of Stuttgart and Sphera,
Evaluation Procedure for Emissions of Volatile Organic Leinfelden-Echterdingen, 2020
Compounds (VVOC, VOC and SVOC) from (http://documentation.gabi-software.com/)
Building Products
IBU 2016
AVV/EWC Institut Bauen und Umwelt eV: General Program
Abfallverzeichnis-Verordnung (AVV)/ European Waste Instructions for the Preparation of EPDs at the Institut
Catalogue (EWC). Commission Decision of 18 Bauen und Umwelt eV Version 1., Berlin: Institut
December 2014 amending Decision 2000/532/EC on Bauen und Umwelt eV, 2016.
the list of waste pursuant to Directive 2008/98/EC of www.ibu-epd.com
the European Parliament and of the Council
Construction Products Regulation (CPR)
Regulation (EU) No 305/2011 Of the European
Parliament and of the Council of 9 March 2011 laying
11 Environmental Product Declaration Pittsburgh Corning Europe NV – FOAMGLAS® T4+
Publisher
Institut Bauen und Umwelt e.V. Tel +49 (0)30 3087748- 0
Panoramastr. 1 Fax +49 (0)30 3087748- 29
10178 Berlin Mail info@ibu-epd.com
Germany Web www.ibu-epd.com
Programme holder
Institut Bauen und Umwelt e.V. Tel +49 (0)30 - 3087748- 0
Panoramastr 1 Fax +49 (0)30 – 3087748 - 29
10178 Berlin Mail info@ibu-epd.com
Germany Web www.ibu-epd.com
Author of the Life Cycle
Assessment Tel +49 711 341817-0
Sphera Solutions GmbH Fax +49 711 341817-25
Hauptstraße 111- 113 Mail info@sphera.com
70771 Leinfelden-Echterdingen Web www.sphera.com
Germany
Owner of the Declaration
Pittsburgh Corning Europe NV Tel +32 (0) 13 661721
Albertkade 1 Fax +32 (0) 13 667854
3980 Tessenderlo Mail info@foamglas.dcom
Belgium Web www.foamglas.com
