ENVIRONMENTAL PRODUCT DECLARATION
as per ISO 14025 and EN 15804+A2
Owner of the Declaration Pittsburgh Corning Europe NV
Programme holder Institut Bauen und Umwelt e.V. (IBU)
Publisher Institut Bauen und Umwelt e.V. (IBU)
Declaration number EPD-PCE-20200300-IBB2-EN
Issue date 15.03.2021
Valid to 14.03.2026
FOAMGLAS® T3+
Pittsburgh Corning Europe NV
www.ibu-epd.com | https://epd-online.com
Umwelt Produktdeklaration Name des Herstellers – Name des Produkts
1. General Information
Pittsburgh Corning Europe NV FOAMGLAS® T3+
Programme holder Owner of the declaration
IBU – Institut Bauen und Umwelt e.V. Pittsburgh Corning Europe NV
Panoramastr. 1 Albertkade 1
10178 Berlin B-3980 Tessenderlo
Germany Belgium
Declaration number Declared product / declared unit
EPD-PCE-20200300-IBB2-EN FOAMGLAS® T3+ / declared unit 1 kg uncoated
cellular glass insulation material
This declaration is based on the product Scope:
category rules: This document refers to the production of 1 kg
Mineral insulating materials, 12.2018 uncoated "FOAMGLAS® T3+" cellular glass
(PCR checked and approved by the SVR) manufactured in Belgium at Tessenderlo and in Czech
Republic at the Klasterec production facilities of
Pittsburgh Corning Europe NV. The reference year of
Issue date
production is 2019. The environmental impacts of the
15.03.2021
coated product "FOAMGLAS® T3+ in boards & blocks"
are to be assessed with the help of a markup factor in
Valid to the amount of 0.8% for Global Warming Potential.
14.03.2026
The owner of the declaration shall be liable for the
underlying information and evidence; the IBU shall not
be liable with respect to manufacturer information, life
cycle assessment data and evidences.
The EPD was created according to the specifications
of EN 15804+A2. In the following, the standard will be
simplified as EN 15804.
Verification
The standard EN 15804 serves as the core PCR
Independent verification of the declaration and data
according to ISO 14025:2011
Dipl. Ing. Hans Peters internally x externally
(chairman of Institut Bauen und Umwelt e.V.)
Dr. Alexander Röder Matthias Klingler
(Managing Director Institut Bauen und Umwelt e.V.)) (Independent verifier)
2. Product
2.1 Product description/Product definition (DOP) is taking into consideration EN 13167:2015
FOAMGLAS® T3+ is an insulation product for buildings Thermal insulation products for buildings – Factory
made of cellular glass. It is applied to the desired made cellular glass (CG) products – Specification
dimensions in the form of slabs, panels, or other and the CE-marking.
specific elements. The FOAMGLAS® T3+ is in general
unfaced as a slab. In some cases, depending on the For the application and use the respective national
end-use, the slabs can be faced with bitumen on the provisions apply.
top with a PE-foil (e.g. READY, BOARDS) or a white
mineral liner (ROOFBLOCK, ROOF BOARDS). Also, 2.2 Application
on the bottom, the white mineral liner can be applied FOAMGLAS® T3+ products are used for roof, facades,
(cf. BOARDS). interior, in contact with the ground, or specific
insulation.
The product is declared with a density of 95 kg/m³
(±15%) and is supplied in thicknesses of 40 mm to 200 2.3 Technical Data
mm. The technical specifications of FOAMGLAS® T3+
within the scope of this EPD and within the CE
For the placing on the market of the product marking, is according to EN 13167 and EN 14305.
FOAMGLAS® T3+ in the European Union/European
Free Trade Association (EU/EFTA) (with the exception Voluntary data: CEN KEYMARK certificate n°001-BK-
of Switzerland) Construction Products Regulation 516-001; ATG H539; KOMO-CTG100-9; SIA CH672-
(CPR) applies. The product declaration of performance
2 Environmental Product Declaration Pittsburgh Corning Europe NV – FOAMGLAS® T3+
13; ACERMI16-023-1179; Natureplus n°Zt-PCE-0406-
1101-101 1) This product/article/at least one partial article
contains substances listed in the ECHA candidate
Technical data according EN 13167 list (date: 19.01.2021) exceeding 0.1 percentage by
Name Value Unit mass: no
Thermal conductivity λD 0.036 W/(mK)
Water vapour diffusion resistance ∞ 2) This product/article/at least one partial article
-
factor µ = ∞ (infinite being > 40000) (infinite) contains other CMR substances in categories 1A or 1B
Gross density 95 kg/m3 which are not on the candidate list, exceeding 0.1
Compressive strength 0.5 N/mm2 percentage by mass: no
Reaction to fire Class A1
Dimensional stability at 70°C/95%RH (≤0.5mm 3) Biocide products were added to this construction
DS70/90 ) product or it has been treated with biocide products
Water absorption (short/long) ≤ 0.5 kg/m² (this then concerns a treated product as defined by the
(EU) Ordinance on Biocide Products No.
Point load PL ≤ 1.5 mm
528/2012): no
BS ≥
Bending Strength kPa
450
2.6 Manufacture
CC(1.5/1
Compressive creep (long behaviour) kPa The product is made following the protocol of the
/50)225
company. All glass constituents (recycled glass, sand,
sodium carbonate, feldspar, sodium sulfate, sodium
nitrate, iron oxide, and FOAMGLAS®-scrap) are melted
(at ca. 1250°C) in the furnace and drawn into the
shape of a thin-walled tube to enable efficient grinding.
2.4 Delivery status
Melted glass from the melter furnace is put in grinders
FOAMGLAS® T3+ are available in the following
to produce fine glass powder. In the grinding process,
thicknesses from 40 to 200 mm
additives are added so that afterwards, glass foaming
FOAMGLAS® T3+ are available in the following
processes can be envisaged. In the foaming furnace,
dimensions:
cellular glass blocks are made in moulds by heating
- Slabs & Blocks: 600x450mm; 300x450mm
(sintering towards ca 850°C) the glass powder after the
- Boards: 1200x600mm
grinding process. After the foaming process, the
Other dimensions are available on request.
annealing process starts by moving the foamed blocks
on the lehr where they cool according to a precisely
2.5 Base materials/Ancillary materials
determined curve. The cooled blocks are cut into
The main constituents of the product or its
rectangular blocks and if necessary, ground or cut to
components are:
thinner sizes. The produced material is released,
- Sand 15%
labelled, marked, and packed for commercialisation
- Feldspar 20%
and various end-use applications (roof, wall, facade
- Recycled content (glass/scrap) 50% to 60%
and other construction elements).
- Others 5% to 15%
3 Environmental Product Declaration Pittsburgh Corning Europe NV – FOAMGLAS® T3+
1 Mixing and batching of the raw materials: Recycled 10 The FOAMGLAS® blocks pass through an
glass, feldspar, sodium carbonate, iron oxide, annealing oven to allow carefully controlled cooling
manganese oxide, sodium sulphate, sodium nitrate. without thermal stress.
2 The melting furnace has a constant temperature of 11 The blocks are cut to size and sorted by batch.
1250°C. Production waste is recycled.
3 Molten glass is drawn out of the furnace. 12 FOAMGLAS® slabs are then packaged, labelled
4 Control room for monitoring the production. and palletized.
5 The glass is drawn off and falls onto the conveyor 13 Finished FOAMGLAS® products are stored and
band where it cools down before entering the ball mill. prepared for transport.
6 Addition of "carbon black".
7 Ball mill grinds all ingredients into a fine powder Quality assurance
before putting them into stainless steel moulds. Quality is assured through internal and external
8 The filled moulds pass through a cellulating oven monitoring. The product complies with the Declaration
(foaming furnace) with a temperature of 850°C. of Performance. It also bears the CEN Keymark
This is where the material gains its unique cell
structure.
9 Energy recovery of heat.
4 Environmental Product Declaration Pittsburgh Corning Europe NV – FOAMGLAS® T3+
2.7 Environment and health during Committee for the Health-Related Evaluation of
manufacturing Building Products (AgBB scheme). (emissions test as
During the entire manufacturing process, no other per EN 16516)
health protection measures extending beyond the
legally specified industrial protection measures for 2.12 Reference service life
commercial enterprises are needed. Health and safety Material composition does not alter during use. The
management is in accordance with EN ISO 45001 and declaration of the service life (RSL) is 100 years.
OHSAS 18001. FOAMGLAS® products can be used practically
indefinitely when used as designated. FOAMGLAS®
Environmental protection during manufacturing: products are impervious to moisture, ants, acids and
Water/Soil: chemicals.
Water incurred during manufacturing and plant
cleaning is treated mechanically in a waste water
treatment system on the plant site and re-used in the 2.13 Extraordinary effects
production process. Waste water corresponds with the
local specifications and the low Al O suspended Fire
2 3
particles contained in the waste water support waste Unfaced FOAMGLAS® is classified as Euro class A1 in
water cleaning. accordance with EN 13501-1 Class A1 building
products do not display any hazard potential regarding
Noise: smoke development, flammability or burning drips.
The noise emissions into the environment by Faced FOAMGLAS®, in form of faced blocks or boards
production equipment fall short of the permissible limit consist of core material class A1 with a facing
values. classified class E in accordance with EN 13501-1
The requirements concerning quality management, Fire protection
environmental management and energy management Name Value
are complied with: (EN ISO 9001, EN ISO 14001, EN Building material class A1
ISO 50001) Burning droplets zero
Smoke gas development zero
2.8 Product processing/Installation
Recommendations on product processing depend on Water
the respective product and system and are outlined in Thanks to its closed-cell structure, exposure to
the respective documentation and data sheets moisture cannot impair the insulating properties of
(available at www.foamglas.com). FOAMGLAS®. Even when exposed to water over long
The product does not contain any concentrations of periods of time (e.g. floods), the insulating material
substances known to be hazardous to health. Dust remains intact.
incurred during sawing is inert and non-crystalline.
Depending on requirements, FOAMGLAS® elements Mechanical destruction
are applied dry or using mineral or bituminous FOAMGLAS® is extremely resilient in all respects, and
adhesives. there is no risk of mechanical destruction if used as
The insulating slabs are staggered and butt-joined with designated. It does not represent any environmental
or without glue. The professional liability associations' hazards thanks to its mineral composition. See
rules apply. When applying the products under review, Material Safety Data Sheets for FOAMGLAS® and
conventional industrial protection measures must be natureplus certificate.
observed in accordance with information supplied by
the manufacturer.
According to the present state of knowledge, hazards 2.14 Re-use phase
for water, air and soil cannot arise if FOAMGLAS® is When sorted, the declared products can be re-ground
applied as designated and re-used as additives in the manufacture of
FOAMGLAS® (material recycling). Otherwise sorted
2.9 Packaging products - even those still bearing adhesive – are
Re-usable wooden pallets, PE shrink foil and suitable for re-use as filling material for brick
cardboard elements serve as packaging material. production, civil engineering, road construction or for
Packaging material (PE foil and cardboard) is disposed sound barriers, for example (material recycling). Within
of on the building site. Thermal utilisation takes place. the re-use of existing surface insulated with
FOAMGLAS®, the existing layer can be topped with a
new layer of FOAMGLAS®
2.10 Condition of use
Material composition does not alter during use. 2.15 Disposal
FOAMGLAS® T3+ products can be used practically Where the recycling options referred to above are not
indefinitely when used as designated. They are practical, foam glass residue incurred on the
impervious to moisture, pests, acids and chemicals. construction site as well as residue from
deconstruction can be easily deposited without
2.11 Environment and health during use preliminary treatment in Class I landfills thanks to their
Ingredients: No particular features regarding the non-leaching mineral components. Packaging can be
material composition for the period of use. In utilised thermally. The waste code number as per the
accordance with official emission measurements for List of Wastes Ordinance (AVV/EWC) for
indoor air, FOAMGLAS® T3+ is an insulating material FOAMGLAS® (uncontaminated) is 17 06 04. In
which does not display VOC (volatile organic combination with bituminous waterproofing substances
compounds) or carcinogenic emissions after 3 and 28
days (see section 7.2) according to the German
5 Environmental Product Declaration Pittsburgh Corning Europe NV – FOAMGLAS® T3+
and adhesive, waste code number 17 09 04 is for 2.16 Further information
unsorted waste. Further information on FOAMGLAS® insulating
materials are available online on the manufacturer's
website: www.foamglas.com.
3. LCA: Calculation rules
3.1 Declared Unit framework of the LCA. This recycled glass is
The Declaration refers to the life cycle of 1kg regarded as a waste product and is therefore
FOAMGLAS® T3 +. The gross density of the product
calculated as input without loads.
is 95 kg / m³ ± 15%
 EU region datasets for grid electricity and
thermal energy from natural gas were used
Declared unit
Name Value Unit for taking potential credits.
Declared unit 1 kg  The calorific values (incineration) of
Gross density 95 kg/m3 packaging material considered are corrugated
conversion factor [Mass/Declared 1 - board: 14 MJ/kg, polyethene-film (PE): 40
Unit]
MJ/kg and wooden pallet: 16 MJ/kg.
 For the calculation of biogenic content, the
biotic carbon dioxide considered is corrugated
3.2 System boundary board: 1.57 kg CO 2/kg corrugated board,
Type of EPD: Cradle to Grave with options, modules wooden pallet: 1.36 kg CO /kg wooden pallet.
2
C1-C4, and module D (A1-A3, C, D and additional
modules)
The LCA addresses the life cycle stage of production,
3.4 Cut-off criteria
installation, end-of-life (EoL) and potential benefits
In the assessment, all available data from the
beyond the system boundaries.
production process are considered, ie all raw materials
The product stage comprises of modules A1 (raw
used, utilized thermal energy, and electric power
material supply), A2 (transport) and A3 (production).
consumption using best available LCI datasets. The
The following individual processes were included in the
material and energy flow with a share of less than 1%
product stage A1- A3 of production:
(based on the total mass of the product) were
 Processes for providing preliminary products
neglected. The sum of the excluded material flows
and energy does not exceed 5% of mass, energy or environmental
 Transporting the raw materials and relevance. Machinery, plants and infrastructure
preliminary materials to the plant required in the manufacturing process were not
 The manufacturing process in the plant considered.
including energy-related expenses, disposal
3.5 Background data
of residual materials and emissions
The software system "GaBi 9 2020" developed by
 Production of packaging thinkstep AG - was used to model and assess the life
cycle. The data sets contained in the GaBi database
Module A4 takes into account the transportation of are documented in the online GaBi documentation
product to the construction site. The treatment of the (2020). These datasets were applied for energy,
packaging materials is assigned to module A5 . transport, preliminary products and auxiliaries. No data
Module C1 takes into accounts the de-construction or records other than GaBi databases were used.
demolition of the product before taking it for
treatment/disposal through means of transportation The Life Cycle Assessment was carried out for the
(module C2). Module C3 is the waste processing of the geographical scope of Belgium (Tessenderlo plant)
product before recycling/recovery/reuse. Landfilling and Czech Republic (Klasterec plant). If no country-
with residual materials is assigned to module C4 . specific data sets were available, comparable data
Module D accounts for the potential credits resulting sets, preferably DE or EU-28 were used. For the
from the thermal and electrical energy generated when Pittsburgh Corning Europe NV Tessenderlo plant,
burning packaging materials in module A5 (energy renewable energy mix of European Green 2019 was
substitution). applied. For the Klasterec plant, electricity from
There are 3 EoL scenarios in the study: Landfill, Reuse hydropower (Slovakia region) was applied. Electricity
and Recycling. Module D/2 takes into account potential source for both plants was provided along with valid
credits for 100% reuse of material and module D/3 energy certificates.
considers potential credits for replacing kaolin in the
brick industry. 3.6 Data quality
All background datasets were taken from the GaBi 9
2020 software database. The background data used
3.3 Estimates and assumptions for the LCA was last revised less than 4 years
ago. Pittsburgh Corning Europe NV supplied current
 An average product based on production
primary production data for 2019. This production data
volume in Tessenderlo and Klasterec was
was examined for plausibility. The corresponding
calculated.
datasets were available in the database for all
 In the product system, external cullet or waste
preliminary products used. The data quality can be
glass is used as a secondary
regarded as very good.
material/preliminary product within the
6 Environmental Product Declaration Pittsburgh Corning Europe NV – FOAMGLAS® T3+
3.7 Period under review 3.9 Comparability
The data in this LCA are based on primary data on Basically, a comparison or an evaluation of EPD data
production in 2019 supplied by Pittsburgh Corning is only possible if all the data sets to be compared
Europe NV. The volumes of raw materials, energy, were created according to EN 15804 and the building
auxiliaries and consumables used are considered as context, respectively the product-specific
average annual values. characteristics of performance, are taken into account.
3.8 Allocation The background database is used from GaBi
The FOAMGLAS® products are produced in a software, version 9.5 and Service pack number of the
separate production line, with no co-products, hence database used is 40
no co-product allocation rules were applied.
4. LCA: Scenarios and additional technical information
Characteristic product properties Recycling potential of FOAMGLAS 0.44 kg
Information on biogenic Carbon
The biogenic carbon content quantifies the amount of
biogenic carbon in a construction product leaving the
factory gate
Information on Biogenic Carbon Content for the
declared unit
Name Value Unit
Biogenic Carbon Content in product 0 kg C
Biogenic Carbon Content in
0.015 kg C
accompanying packaging
All the following technical scenario information is given
for the declared unit (i.e., 1 kg FOAMGLAS® product)
Transport to the building site (A4)
Name Value Unit
Transport distance 350 km
Capacity utilisation (including empty
61 %
runs)
Installation into the building (A5)
Name Value Unit
Output substances following waste
0.009 kg
treatment on site (Paper)
Output substances following waste
0.022 kg
treatment on site (Plastic)
Output substances following waste
0.029 kg
treatment on site (Wood)
End of life (C1 - C4)
There are 3 End-of-Life scenarios considered in the
study,
Scenario 1: Landfill
Scenario 2: Reuse
Scenario 3: Recycle
Name Value Unit
Landfilling 1 kg
Reuse 1 kg
Recycled 0.44 kg
Reuse, recovery and/or recycling potentials (D),
relevant scenario information
Name Value Unit
Thermal utilization of cardboard from
0.009 kg
the packaging
Thermal utilization of PE Film (plastic)
0.022 kg
from the packaging
Thermal utilization of wooden pallets
0.029 kg
from the packaging
7 Environmental Product Declaration Pittsburgh Corning Europe NV – FOAMGLAS® T3+
5. LCA: Results
End-of-Life scenarios: 1. Landfill, 2. Reuse, 3. Recycling
C3 / 2 - Waste processing for reuse
C3 / 3 - Waste processing for recycling
C4 / 1 - Landfill
D - Potential benefits for thermal utilization of packaging materials
D / 2- Potential benefits for reuse
D / 3- Potential benefits for recycling
DESCRIPTION OF THE SYSTEM BOUNDARY (X = INCLUDED IN LCA; ND = MODULE OR INDICATOR NOT
DECLARED; MNR = MODULE NOT RELEVANT)
BENEFITS AND
CONSTRUCTI LOADS
PRODUCT STAGE ON PROCESS USE STAGE END OF LIFE STAGE BEYOND THE
STAGE SYSTEM
BOUNDARIES
8 Environmental Product Declaration Pittsburgh Corning Europe NV – FOAMGLAS® T3+
lairetam
waR
ylppus tropsnarT
gnirutcafunaM
eht
morf
tropsnarT
etis
eht
ot
etag
ylbmessA esU
ecnanetniaM
riapeR
tnemecalpeR tnemhsibrufeR
ygrene
lanoitarepO esu
retaw
lanoitarepO esu
noitcurtsnoc-eD
noitilomed tropsnarT
gnissecorp
etsaW
lasopsiD -esueR -yrevoceR -gnilcyceR laitnetop
A1 A2 A3 A4 A5 B1 B2 B3 B4 B5 B6 B7 C1 C2 C3 C4 D
X X X X X ND ND MNR MNR MNR ND ND X X X X X
RESULTS OF THE LCA - ENVIRONMENTAL IMPACT according to EN 15804+A2: 1 kg FOAMGLAS® T3+
Core Indicator Unit A1-A3 A4 A5 C1 C2 C3/2 C3/3 C4/1 D D/2 D/3
GWP-total [kg CO2-Eq.] 1.45E+0 2.96E-2 1.23E-1 6.47E-4 2.35E-3 0.00E+0 1.95E-3 1.53E-2 -5.13E-2 -1.45E+0 -1.43E-1
GWP-fossil [kg CO2-Eq.] 1.50E+0 2.80E-2 5.79E-2 6.40E-4 2.23E-3 0.00E+0 1.93E-3 1.52E-2 -5.12E-2 -1.50E+0 -1.43E-1
GWP-biogenic [kg CO2-Eq.] -4.72E-2 1.33E-3 6.53E-2 1.93E-6 1.06E-4 0.00E+0 1.70E-5 4.86E-5 -1.17E-4 4.72E-2 -2.25E-4
GWP-luluc [kg CO2-Eq.] 8.48E-4 2.28E-4 3.94E-6 4.99E-6 1.81E-5 0.00E+0 2.80E-6 4.37E-5 -3.35E-5 -8.48E-4 -3.43E-5
ODP [kg CFC11-Eq.] 1.01E-13 3.38E-18 3.75E-17 7.41E-20 2.68E-19 0.00E+0 4.25E-17 5.62E-17 -4.98E-16 -1.01E-13 -2.61E-16
AP [mol H+-Eq.] 4.77E-3 2.95E-5 2.14E-5 3.09E-6 7.17E-6 0.00E+0 4.26E-6 1.09E-4 -6.91E-5 -4.77E-3 -1.32E-4
EP-freshwater [kg P4-Eq.] 2.73E-5 8.55E-8 5.99E-9 1.87E-9 6.79E-9 0.00E+0 5.16E-9 2.60E-8 -6.16E-8 -2.73E-5 -5.23E-8
EP-marine [kg N-Eq.] 1.79E-3 8.74E-6 6.07E-6 1.44E-6 3.23E-6 0.00E+0 9.47E-7 2.80E-5 -1.81E-5 -1.79E-3 -4.75E-5
EP-terrestrial [mol N-Eq.] 1.89E-2 1.05E-4 9.84E-5 1.59E-5 3.61E-5 0.00E+0 9.95E-6 3.08E-4 -1.95E-4 -1.89E-2 -5.23E-4
POCP [kg NMVOC-Eq.] 4.13E-3 2.40E-5 1.65E-5 4.03E-6 6.33E-6 0.00E+0 2.59E-6 8.48E-5 -5.23E-5 -4.13E-3 -1.44E-4
ADPE [kg Sb-Eq.] 2.38E-7 2.02E-9 5.33E-10 4.42E-11 1.60E-10 0.00E+0 5.59E-10 1.36E-9 -8.00E-9 -2.38E-7 -1.01E-8
ADPF [MJ] 2.30E+1 3.74E-1 4.19E-2 8.20E-3 2.97E-2 0.00E+0 3.39E-2 1.99E-1 -8.66E-1 -2.30E+1 -2.35E+0
[m³ world-Eq
WDP 1.23E-1 2.51E-4 1.29E-2 5.51E-6 2.00E-5 0.00E+0 4.21E-4 1.59E-3 -4.94E-3 -1.23E-1 -2.65E-3
deprived]
GWP = Global warming potential; ODP = Depletion potential of the stratospheric ozone layer; AP = Acidification potential of land and water; EP =
Caption Eutrophication potential; POCP = Formation potential of tropospheric ozone photochemical oxidants; ADPE = Abiotic depletion potential for non-
fossil resources; ADPF = Abiotic depletion potential for fossil resources; WDP = Water (user) deprivation potential
RESULTS OF THE LCA - INDICATORS TO DESCRIBE RESOURCE USE according to EN 15804+A2: 1 kg
FOAMGLAS® T3+
Indicator Unit A1-A3 A4 A5 C1 C2 C3/2 C3/3 C4/1 D D/2 D/3
PERE [MJ] 1.33E+1 2.10E-2 6.10E-1 4.61E-4 1.67E-3 0.00E+0 1.50E-2 2.61E-2 -1.77E-1 -1.33E+1 -9.55E-2
PERM [MJ] 6.00E-1 0.00E+0 -6.00E-1 0.00E+0 0.00E+0 0.00E+0 0.00E+0 0.00E+0 0.00E+0 -6.00E-1 0.00E+0
PERT [MJ] 1.39E+1 2.10E-2 1.00E-2 4.61E-4 1.67E-3 0.00E+0 1.50E-2 2.61E-2 -1.77E-1 -1.39E+1 -9.55E-2
PENRE [MJ] 2.21E+1 3.75E-1 9.32E-1 8.21E-3 2.98E-2 0.00E+0 3.40E-2 1.99E-1 -8.66E-1 -2.21E+1 -2.35E+0
PENRM [MJ] 8.90E-1 0.00E+0 -8.90E-1 0.00E+0 0.00E+0 0.00E+0 0.00E+0 0.00E+0 0.00E+0 -8.90E-1 0.00E+0
PENRT [MJ] 2.30E+1 3.75E-1 4.20E-2 8.21E-3 2.98E-2 0.00E+0 3.40E-2 1.99E-1 -8.66E-1 -2.30E+1 -2.35E+0
SM [kg] 5.60E-1 0.00E+0 0.00E+0 0.00E+0 0.00E+0 0.00E+0 0.00E+0 0.00E+0 0.00E+0 0.00E+0 0.00E+0
RSF [MJ] 0.00E+0 0.00E+0 0.00E+0 0.00E+0 0.00E+0 0.00E+0 0.00E+0 0.00E+0 0.00E+0 0.00E+0 0.00E+0
NRSF [MJ] 0.00E+0 0.00E+0 0.00E+0 0.00E+0 0.00E+0 0.00E+0 0.00E+0 0.00E+0 0.00E+0 0.00E+0 0.00E+0
FW [m³] 3.94E-2 2.44E-5 3.06E-4 5.34E-7 1.94E-6 0.00E+0 1.74E-5 5.02E-5 -2.05E-4 -3.94E-2 -1.12E-4
PERE = Use of renewable primary energy excluding renewable primary energy resources used as raw materials; PERM = Use of
renewable primary energy resources used as raw materials; PERT = Total use of renewable primary energy resources; PENRE = Use of
non-renewable primary energy excluding non-renewable primary energy resources used as raw materials; PENRM = Use of non-
Caption
renewable primary energy resources used as raw materials; PENRT = Total use of non-renewable primary energy resources; SM = Use
of secondary material; RSF = Use of renewable secondary fuels; NRSF = Use of non-renewable secondary fuels; FW = Use of net fresh
water
RESULTS OF THE LCA – WASTE CATEGORIES AND OUTPUT FLOWS according to EN 15804+A2:
1 kg FOAMGLAS® T3+
Indicator Unit A1-A3 A4 A5 C1 C2 C3/2 C3/3 C4/1 D D/2 D/3
HWD [kg] 4.96E-8 1.74E-8 1.14E-10 3.82E-10 1.39E-9 0.00E+0 1.41E-11 3.03E-9 -3.44E-10 -4.96E-8 -1.98E-9
NHWD [kg] 4.12E-2 5.74E-5 6.69E-3 1.26E-6 4.56E-6 0.00E+0 2.41E-5 1.00E+0 -3.86E-4 -4.12E-2 -6.23E-4
RWD [kg] 1.09E-4 4.64E-7 1.85E-6 1.02E-8 3.68E-8 0.00E+0 5.15E-6 2.26E-6 -6.03E-5 -1.09E-4 -3.14E-5
CRU [kg] 0.00E+0 0.00E+0 0.00E+0 0.00E+0 0.00E+0 1.00E+0 0.00E+0 0.00E+0 0.00E+0 0.00E+0 0.00E+0
MFR [kg] 0.00E+0 0.00E+0 0.00E+0 0.00E+0 0.00E+0 0.00E+0 4.40E-1 0.00E+0 0.00E+0 0.00E+0 0.00E+0
MER [kg] 0.00E+0 0.00E+0 6.09E-2 0.00E+0 0.00E+0 0.00E+0 0.00E+0 0.00E+0 0.00E+0 0.00E+0 0.00E+0
EEE [MJ] 0.00E+0 0.00E+0 2.02E-1 0.00E+0 0.00E+0 0.00E+0 0.00E+0 0.00E+0 0.00E+0 0.00E+0 0.00E+0
EET [MJ] 0.00E+0 0.00E+0 4.15E-1 0.00E+0 0.00E+0 0.00E+0 0.00E+0 0.00E+0 0.00E+0 0.00E+0 0.00E+0
HWD = Hazardous waste disposed; NHWD = Non-hazardous waste disposed; RWD = Radioactive waste disposed; CRU = Components
Caption for re-use; MFR = Materials for recycling; MER = Materials for energy recovery; EEE = Exported electrical energy; EEE = Exported
thermal energy
RESULTS OF THE LCA – additional impact categories according to EN 15804+A2-optional:
1 kg FOAMGLAS® T3+
Indicator Unit A1-A3 A4 A5 C1 C2 C3/2 C3/3 C4/1 D D/2 D/3
[Disease
PM 4.81E-8 1.73E-10 1.88E-10 3.47E-11 3.92E-11 0.00E+0 3.58E-11 1.35E-9 -5.88E-10 -4.81E-8 -7.10E-9
Incidence]
[kBq U235-
IRP 1.51E-2 6.71E-5 2.25E-4 1.47E-6 5.33E-6 0.00E+0 8.45E-4 2.32E-4 -9.89E-3 -1.51E-2 -5.13E-3
Eq.]
ETP-fw [CTUe] 3.78E+1 2.65E-1 1.68E-2 5.80E-3 2.10E-2 0.00E+0 1.45E-2 1.14E-1 -1.75E-1 -3.78E+1 -1.29E-1
HTP-c [CTUh] 8.62E-10 5.54E-12 1.29E-12 1.21E-13 4.40E-13 0.00E+0 4.01E-13 1.68E-11 -7.96E-12 -8.62E-10 -1.76E-11
HTP-nc [CTUh] 3.63E-8 2.87E-10 1.03E-10 7.28E-12 2.58E-11 0.00E+0 1.48E-11 1.86E-9 -2.96E-10 -3.63E-8 -6.73E-10
SQP [-] 1.71E+1 1.31E-1 1.22E-2 2.88E-3 1.04E-2 0.00E+0 1.08E-2 4.15E-2 -1.27E-1 -1.71E+1 -7.61E-2
PM = Potential incidence of disease due to PM emissions; IR = Potential Human exposure efficiency relative to U235; ETP-fw = Potential
Caption comparative Toxic Unit for ecosystems; HTP-c = Potential comparative Toxic Unit for humans (cancerogenic); HTP-nc = Potential
comparative Toxic Unit for humans (not cancerogenic); SQP = Potential soil quality index
The transportation distance to waste processing system (module C2) is considered as 30 km. Specifically, for
scenario 3, ie recycling, the transportation distance to the brick industry is 100 km, hence multiply the results in
module C2 by 3.33 (i.e.,100/30) to get the result for 100 km.
The environmental impacts of the coated product are to be assessed with the help of a markup factor in the
amount of 0.8% for Global Warming Potential and for all LCA results, the maximum deviation is 5.44%.
Disclaimer 1 - for the indicator IRPT This impact category deals mainly with the eventual impact of low dose
ionizing radiation on human health of the nuclear fuel cycle. It does not consider effects due to possible nuclear
accidents, occupational exposure nor due to radioactive waste disposal in underground facilities. Potential
ionizing radiation from the soil, from radon and some construction materials is also not measured by this indicator.
Disclaimer 2 - The results of environmental impact indicators ADPE, ADPF, WDP, ETP-fw, HTP-c, HTP-nc, SQP
shall be used with care as the uncertainties on these results are high or as there is limited experience with the
indicator.
6. LCA: Interpretation
The contributions from module A1 (raw materials) and Eutrophication -freshwater. The relevant contributor
A3 (energy) dominate in climate change impact. The (25% - 50%) for most of the impact categories are
modules A4, A5, C1, C2, C3 and C4 contributes less. Sodium carbonate and Feldspar with around 40%
The credits in this study i.e. module D result from the contribution in Resource use (energy carriers) and
incineration of packaging materials. Module D/2 credit Total use of renewable and non-renewable primary
is highest as the 100% manufacturing impacts of the energy resources and 50% contribution in Climate
product are taken as a credit for its 100% reuse. change and Eutrophication freshwater. The other
relevant contributor is iron oxide. Manganese dioxide
The significant contributor (> 50%) among all the raw contributes 60% in Resource use (mineral and metals),
materials is Sodium carbonate, with around 70% as the use of manganese ore for its production leads to
impact in Photochemical ozone formation and net depletion of mineral and metal resource.
freshwater use; and around 77% contribution in
7. Requisite evidence
7.1 Bio-persistence 7.3 Leaching
FOAMGLAS® products do not contain fibres and also The ELUAT-tests on FOAMGLAS® products according
biocides. the ICP-MS tests method ISO 17294-2 result below
limits (test report No 2017-382 conducted by Indikator
7.2 Radioactivity laboratory). The AOX/EOX halogen (ISO 9562) value
The radon diffusion coefficient FOAMGLAS® products is zero (test report No 2017-380 Indikator laboratory).
is less than 10-11 testreport No RAD 592 conducted at
LaRUC Uni Cantabria of Spain – RiSE/SP Technical 7.4 Formaldehyde and VOC emissions
Research Institute of Sweden, Prague Technical tested according EN 16516, the formaldehyde & VOC
University of Czech Republic. indoor emissions results for FOAMGLAS® products
(Laboratory Bremer Umweltinstitut No H3989 at
9 Environmental Product Declaration Pittsburgh Corning Europe NV – FOAMGLAS® T3+
Bremen, Germany; Laboratoire Excell at Mérignac in VOC without NIK <5 μg/m3
France, No 192-17367; VITO SERVACO at Mol, Carcinogenic Substances <1 μg/m3
Belgium No ML02001-28R): Formaldehyde <1 μg/m3
AgBB overview of results (3 days [µg/m³])
Name Value Unit
TVOC (C6 - C16) <5 μg/m3
Sum SVOC (C16 - C22) <5 μg/m3
AgBB overview of results (28 days [µg/m³]) R (dimensionless) 0
Name Value Unit VOC without NIK <5 μg/m3
TVOC (C6 - C16) <5 μg/m3
Carcinogenic Substances <1 μg/m3
Sum SVOC (C16 - C22) <5 μg/m3
Formaldehyde <1 μg/m3
R (dimensionless) 0
8. References
STANDARDS the product category of construction products
(EN 15804:2012+A2:2019)
DIN 4102-17
DIN 4102-17:2017-12 Fire behaviour of building EN 16516
materials and building components - Part 17: Melting EN 16516:2020-10 Construction products: Assessment
point of mineral wool insulating materials - Terms and of release of dangerous substances. Determination of
definitions, requirements and test emissions into indoor air
EN ISO 9001 EN ISO 17294-2
EN ISO 9001:2015-11 Quality management systems – EN ISO 17294-2:2017-01 Water quality - Application of
Requirements inductively coupled plasma mass spectrometry (ICP-
MS) - Part 2: Determination of selected elements
EN ISO 9562 including uranium isotopes
EN ISO 9562:2005-02 Water quality - Determination of
adsorbable organically bound halogens (AOX) EN ISO 45001
EN ISO 45001:2018-06 Occupational Health and
EN 13167 Safety Assessment Series (OHSAS) 18001:2007
EN 13167:2012+A1:2015/prA2:2018 Thermal
insulation products for buildings - Factory made EN ISO 50001
cellular glass (CG) products EN ISO 50001:2018-12 Energy management systems
- Requirements with guidance for use
EN 13501-1
EN 13501-1:2019-05, Fire classification of construction Product Category Rules, Part B: Guidelines for
products and building elements - Part 1: Classification building-related products and services, Part B:
using data from reaction to fire tests Requirements to be met by the EPD for PCR Mineral
Insulating Materials, Institut Bauen und Umwelt eV,
EN ISO 14001 www.bau-umwelt.com, 2018, version 1.1
EN ISO 14001:2015-11 Environmental management
systems - Requirements with guidance for use Product Category Rules for Construction Products,
Part A: Calculation rules for the life cycle assessment
EN ISO 14025 and requirements on the background Report according
EN ISO 14025:2011-10 Environmental labels and to EN 15804+A2:2019, 2020, version 1.0
declarations - Type III environmental declarations -
Principles and procedures (ISO 14025:2006) CERTIFICATES
EN ISO 14040 CEN Keymark Certificate n°001-BK-516-001; ATG
EN ISO 14040:2021-02 Environmental management - H539; KOMO-CTG100-9; SIA CH672-13; ACERMI16-
Life cycle assessment - Principles and framework 023-1179;
(ISO 14040:2006)
ECHA candidate list
EN ISO 14044 Candidate List substances in articles
EN ISO 14044:2021-02 Environmental management - (date: 19.01.2021)
Life cycle assessment - Requirements and guidelines
(ISO 14044:2006 + Amd 1:2017) Natureplus n°Zt-PCE-0406-1101-101
EN 14305 Green Energy Certificate (Klasterec)
EN 14305:2016-03 Thermal insulation for building KLA-renewable energy, Slovak Power Plants,
equipment and industrial installations - Factory made Pittsburgh Corning CR
cellular glass (CG) products
Green Energy Certificate (Tessenderlo)
EN 15804 Bron hernieuwbare energie 2019, Pittsburgh Corning
EN 15804:2020-03 Sustainability of construction works Europe, Luminus Business Team
- Environmental Product Declarations - Core rules for
10 Environmental Product Declaration Pittsburgh Corning Europe NV – FOAMGLAS® T3+
FURTHER REFERENCES down harmonised conditions for the marketing of
construction products and repealing Council Directive
AgBB 89/106/EEC
Ausschuss zur gesundheitlichen Bewertung
von Bauprodukten (2018). Committee for Health- GaBi 9 2020
related Evaluation of Building Products. Requirements Dataset documentation for the software system and
for the Indoor Air Quality in Buildings: Health-related databases, LBP, University of Stuttgart and Sphera,
Evaluation Procedure for Emissions of Volatile Organic Leinfelden-Echterdingen, 2020
Compounds (VVOC, VOC and SVOC) from (http://documentation.gabi-software.com/)
Building Products
IBU 2016
AVV/EWC Institut Bauen und Umwelt eV: General Program
Abfallverzeichnis-Verordnung (AVV)/ European Waste Instructions for the Preparation of EPDs at the Institut
Catalogue (EWC). Commission Decision of 18 Bauen und Umwelt eV Version 1., Berlin: Institut
December 2014 amending Decision 2000/532/EC on Bauen und Umwelt eV, 2016.
the list of waste pursuant to Directive 2008/98/EC of www.ibu-epd.com
the European Parliament and of the Council
Construction Products Regulation (CPR)
Regulation (EU) No 305/2011 Of the European
Parliament and of the Council of 9 March 2011 laying
11 Environmental Product Declaration Pittsburgh Corning Europe NV – FOAMGLAS® T3+
Publisher
Institut Bauen und Umwelt e.V. Tel +49 (0)30 3087748- 0
Panoramastr. 1 Fax +49 (0)30 3087748- 29
10178 Berlin Mail info@ibu-epd.com
Germany Web www.ibu-epd.com
Programme holder
Institut Bauen und Umwelt e.V. Tel +49 (0)30 - 3087748- 0
Panoramastr 1 Fax +49 (0)30 – 3087748 - 29
10178 Berlin Mail info@ibu-epd.com
Germany Web www.ibu-epd.com
Author of the Life Cycle
Assessment Tel +49 (0)711 341817-0
Sphera Solutions GmbH Fax +49 (0)711 341817-25
Hauptstraße 111- 113 Mail info@sphera.com
70771 Leinfelden-Echterdingen Web www.sphera.com
Germany
Owner of the Declaration
Pittsburgh Corning Europe NV Tel +32 (0) 13 661721
Albertkade 1 Fax +32 (0) 13 667854
3980 Tessenderlo Mail info@foamglas.dcom
Belgium Web www.foamglas.com
