ENVIRONMENTAL PRODUCT DECLARATION
as per ISO 14025 and EN 15804+A2
Owner of the Declaration KONE Corporation
Publisher Institut Bauen und Umwelt e.V. (IBU)
Programme holder Institut Bauen und Umwelt e.V. (IBU)
Declaration number EPD-KON-20230579-CBA2-EN
Issue date 22.12.2023
Valid to 29.06.2028
Folding door system 50 / 50E
KONE
www.ibu-epd.com | https://epd-online.com
General Information
KONE Folding door system 50 / 50E
Programme holder Owner of the declaration
IBU – Institut Bauen und Umwelt e.V. KONE Corporation
Hegelplatz 1 Keilasatama 3
10117 Berlin 02150 ESPOO
Germany Finland
Declaration number Declared product / declared unit
EPD-KON-20230579-CBA2-EN 1 piece of the product: KONE folding door 50, consisting of the following
items:
• Drive unit
• Pairs of folding panels
• Hold-open columns
• Floor rail
• Product packaging
This declaration is based on the product category rules: Scope:
Automatic doors, automatic gates, and revolving door systems, This Environmental Product Declaration refers to the KONE folding door
01.08.2021 50. This EPD is also representative for the folding door 50E. The
(PCR checked and approved by the SVR) production site is located in Germany. Green electricity is being used at
this production site.
Issue date Data represents the year 2022.
22.12.2023
The owner of the declaration shall be liable for the underlying information
and evidence; the IBU shall not be liable with respect to manufacturer
information, life cycle assessment data and evidences.
Valid to
29.06.2028 The EPD was created according to the specifications of EN 15804+A2. In
the following, the standard will be simplified as EN 15804.
Verification
The standard EN 15804 serves as the core PCR
Independent verification of the declaration and data according to ISO
14025:2011
internally X externally
Dipl.-Ing. Hans Peters
(Chairman of Institut Bauen und Umwelt e.V.)
Florian Pronold Dr.-Ing. Wolfram Trinius,
(Managing Director Institut Bauen und Umwelt e.V.) (Independent verifier)
1 Environmental Product Declaration - KONE - Folding door system 50 / 50E
Product
Name Value Unit
Product description/Product definition
Opening and closing force maximum 150 N
The folding doors 50 and 50E are thermally separated, with
Opening speed incremental adjustment 10-75 cm/s
particularly slim profiles and a silent, dynamic drive system.
Both versions are particularly suitable where space is restricted. Closing speed incrementally variable 10-50 cm/s
Maximum heights of up to 2.5 metres are possible. Hold-open time 0-180 s
Installed load, frequency 230 V
The folding doors avail of highly efficient thermal separation
Power consumption 250 W
with very good thermal transmittance values (UD values)
Type of protection 20 IP
ranging from 1.7 to max. 2.4 (thermal coefficient) which can be
calculated individually for each door system. In combination Clear opening width maximum 900-2400 mm
with ISO glass, the folding doors ensure good thermal Panel pair weight maximum 90 kg
insulation of external doors. Clear passage height 2100-2500 mm
Double glazing 28 ISO
For the use and application of the product the representative
national provisions apply. The standards which can be applied Performance data of the product with respect to its
are the following: characteristics in accordance with the relevant technical
provision which can be applied are mentioned above.
• EN 18650-1
• EN 18650-2
• EN 16005 Base materials/Ancillary materials
• EN 60335-1 The major material composition including the packaging of the
• ISO 13849-1 product is listed below.
• 2011/65/EU ROHS3 Directive
Name Value Unit
• Machinery Directive 2006/42/EC
Glass 42 %
The CE marking takes into account the proof of conformity with Aluminium 27 %
the respective harmonized standards based on the legal Steel 19 %
provisions above.
Plastic 6 %
Plastic packaging 4 %
Application Electronics 1 %
The folding doors 50 / 50E are used when a large opening Zinc 1 %
width needs to be achieved despite small wall opening
The folding doors include partial articles which contain
dimensions. They are suitable for external and internal doors in
substances listed in the Candidate List of REACH Regulation
narrow passageways, barrier-free access points in public
1907/2006/EC (date: 17.01.2023) exceeding 0.1 percentage by
buildings as well as escape routes and emergency exits. While
mass: yes
opening, the door panel is simultaneously folded and
automatically moved to the side.
• Lead (Pb): 7439-92-1 (CAS-No.) is used in some of the
alloys. The concentration of lead in each individual alloy
Bi-parting opening
does not exceed 4.0%
Both pairs of door panels are synchronously swivelled to the
(by mass).
side and in opposing directions while opening, thereby
permitting a maximum opening width of 2.4 metres.
The Candidate List can be found on the ECHA website
address: https:echa.europa.eu/de/home.
Unilateral opening
For smaller applications: the folding door comprising a single Reference service life
pair of panels permits a maximum opening width of 1.2 metres. The reference service life of folding doors amounts to 10 years
and depends on the application and frequency of use. Regular
Technical Data
maintenance is advised to ensure the life expectancy of 10
years. For repairs and renewals, suitable spare parts are
The automatic folding doors have the following technical
available. The folding doors are tested and certified to EN
properties:
16005, meaning they are designed to withstand a minimum of
1.000.000 cycles.
LCA: Calculation rules
The type of EPD is: cradle to gate with options, modules C1–
Declared Unit C4, and module D (A1–A3 + C + D and additional modules: A4
The declared unit is 1 piece of the product: + A5 + B6)
Name Value Unit
Declared unit 1 pce. Production - Module A1-A3
The product stage includes:
Mass of the entire system 223.03 kg
— A1, raw material extraction, processing and mechanical
treatments, processing of secondary material input (e.g.
recycling processes),
System boundary
2 Environmental Product Declaration - KONE - Folding door system 50 / 50E
— A2, transport to the manufacturer, — C3, waste processing for reuse, recovery and/or recycling;
— A3, manufacturing and assembly including provision of all — C4, disposal; including provision and all transport, provision
materials, products and energy, as well as waste processing up of all materials, products and related energy and water use.
to the end-of waste state. Module D (Benefits and loads beyond the system boundary)
includes:
Construction stage - Modules A4-A5 — D, recycling potentials, expressed as net impacts and
The construction process stage includes: benefits.
— A4, transport to the building site;
— A5, installation into the building; including provision of all Geographic Representativeness
materials, products and energy, as well as waste processing up Land or region, in which the declared product system is
to the end-of waste state or disposal of final residues during the manufactured, used or handled at the end of the product´s
construction process stage. lifespan: Global
Use stage - Module B6
Comparability
The use stage related to the operation of the building includes:
Basically, a comparison or an evaluation of EPD data is only
— B6, operational energy use
possible if all the data sets to be compared were created
according to EN 15804 and the building context, respectively
End-of-life stage– Modules C1-C4 and D
the product-specific characteristics of performance, are taken
The end-of-life stage includes:
into account. Background database: GaBi, SP40
— C1, deconstruction, demolition:
— C2, transport to waste processing;
LCA: Scenarios and additional technical information
Name Value Unit
Characteristic product properties of biogenic carbon
Electricity consumption for 1 year 224.65 kWh
Days per year in use 365 days
Information on describing the biogenic carbon content at
Active mode per day 1,80 h
factory gate
Idle mode per day 22,20 h
Name ValueUnit
Active mode power 16,33 W
kg
Biogenic carbon content in product 0.05 Idle mode power 26,40 W
C
Biogenic carbon content in accompanying 0.08 kg End of life (C1-C4)
packaging C
C1: The product expansion depends on the building. The
Note: 1 kg of biogenic carbon is equivalent to 44/12 kg of CO . product share is so low that no environmental burden is
2
assumed.
C2: Transport to waste management 50 km.
Name Value Unit
Transport to the building site (A4)
Collected separately waste type 214 kg
Name Value Unit
Recycling 106 kg
Litres of fuel (per 1kg) 0.00276 l/100km
Energy recovery 13 kg
Capacity utilisation (including empty runs) 55 %
Landfilling 94.8 kg
Transport distance via medium truck 100 km
The product is transported via truck. The main distribution
The product is disassembled in a recycling process. Material
region is Europe. In order to allow scaling to a specific point of
recycling is then assumed for the metals and electronics. The
installation 100 km are declared.
plastic components are assumed to be incinerated with energy
recovery. Electromechanics and minor proportions of residues
Installation into the building (A5) arising from the recycling process are landfilled.
Name Value Unit Region for the End of Life is: Global.
Waste packaging (paper and plastic) 9,198 kg
Reuse, recovery and/or recycling potentials (D), relevant
scenario information
Reference service life
Name Value Unit
Name Value Unit
Recycling 100 %
Life Span according to the manufacturer 10 a
The collection rate is 100%.
Operational energy use (B6)
3 Environmental Product Declaration - KONE - Folding door system 50 / 50E
LCA: Results
DESCRIPTION OF THE SYSTEM BOUNDARY (X = INCLUDED IN LCA; MND = MODULE OR INDICATOR NOT DECLARED; MNR
= MODULE NOT RELEVANT)
Benefits and
Construction loads beyond
Product stage Use stage End of life stage
process stage the system
boundaries
la ire ta m w a Ry lp p u s tro p s n a rT g n iru tc a fu n a M e h t m o rf tro p s n a rTe tis e h t o t e ta g y lb m e s s A e s U e c n a n e tn ia M ria p e R tn e m e c a lp e R tn e m h s ib ru fe R y g re n e la n o ita re p Oe s u re ta w la n o ita re p Oe s u n o itc u rts n o c -e Dn o itilo m e d tro p s n a rT g n is s e c o rp e ts a W la s o p s iD -e s u e R-y re v o c e R-g n ilc y c e Rla itn e to p
A1 A2 A3 A4 A5 B1 B2 B3 B4 B5 B6 B7 C1 C2 C3 C4 D
X X X X X MND MND MNR MNR MNR X MND X X X X X
RESULTS OF THE LCA - ENVIRONMENTAL IMPACT according to EN 15804+A2: 1 piece Folding Door 50 / 50E
Parameter Unit A1-A3 A4 A5 B6 C1 C2 C3 C4 D
GWP-total kg CO 2 eq 5.05E+02 1.95E+00 2.32E+01 0 0 9.34E-01 3.35E+01 1.45E+00 -1.61E+02
GWP-fossil kg CO 2 eq 5.04E+02 1.87E+00 2.29E+01 0 0 8.93E-01 3.33E+01 1.44E+00 -1.6E+02
GWP-biogenic kg CO 2 eq 8.28E-01 8.6E-02 3.17E-01 0 0 4.1E-02 2.23E-01 5E-03 -1.52E-01
GWP-luluc kg CO 2 eq 3.15E-01 4.44E-05 1E-03 0 0 2.13E-05 2E-03 4E-03 -1.04E-01
ODP kg CFC11 eq 1.67E-09 1.97E-16 1.16E-14 0 0 9.43E-17 1.68E-14 5.33E-15 -6.06E-10
AP mol H+ eq 2.58E+00 2E-03 4E-03 0 0 8.94E-04 6E-03 1E-02 -5.49E-01
EP-freshwater kg P eq 5.68E-04 3.99E-07 1.85E-06 0 0 1.91E-07 2.68E-06 2.47E-06 -1.26E-04
EP-marine kg N eq 5.41E-01 5.94E-04 9.34E-04 0 0 2.84E-04 1E-03 3E-03 -8.3E-02
EP-terrestrial mol N eq 6.03E+00 7E-03 1.9E-02 0 0 3E-03 2.7E-02 2.9E-02 -8.9E-01
kg NMVOC
POCP 1.4E+00 2E-03 3E-03 0 0 8.04E-04 4E-03 8E-03 -2.62E-01
eq
ADPE kg Sb eq 1.3E-02 5.59E-08 1.59E-07 0 0 2.68E-08 2.31E-07 1.29E-07 -4E-03
ADPF MJ 7.26E+03 2.64E+01 1.07E+01 0 0 1.27E+01 1.55E+01 1.89E+01 -2.19E+03
m3 world eq
WDP 4.89E+01 4E-03 2.38E+00 0 0 2E-03 3.43E+00 1.51E-01 -2.33E+01
deprived
GWP = Global warming potential; ODP = Depletion potential of the stratospheric ozone layer; AP = Acidification potential of land and water; EP =
Eutrophication potential; POCP = Formation potential of tropospheric ozone photochemical oxidants; ADPE = Abiotic depletion potential for non-fossil
resources; ADPF = Abiotic depletion potential for fossil resources; WDP = Water (user) deprivation potential)
RESULTS OF THE LCA - INDICATORS TO DESCRIBE RESOURCE USE according to EN 15804+A2: 1 piece Folding Door 50 /
50E
Parameter Unit A1-A3 A4 A5 B6 C1 C2 C3 C4 D
PERE MJ 1.28E+03 8.3E-02 5.35E+00 0 0 4E-02 5.51E+00 2.47E+00 -7.01E+02
PERM MJ 4.06E+00 0 -2.57E+00 0 0 0 -1.49E+00 0 0
PERT MJ 1.28E+03 8.3E-02 2.77E+00 0 0 4E-02 4.02E+00 2.47E+00 -7.01E+02
PENRE MJ 6.62E+03 2.65E+01 3.98E+02 0 0 1.27E+01 2.68E+02 1.89E+01 -2.19E+03
PENRM MJ 6.39E+02 0 -3.87E+02 0 0 0 -2.52E+02 0 0
PENRT MJ 7.26E+03 2.65E+01 1.07E+01 0 0 1.27E+01 1.55E+01 1.89E+01 -2.19E+03
SM kg 7.83E+01 0 0 0 0 0 0 0 0
RSF MJ 0 0 0 0 0 0 0 0 0
NRSF MJ 0 0 0 0 0 0 0 0 0
FW m3 2.95E+00 1.5E-04 5.7E-02 0 0 7.16E-05 8.2E-02 5E-03 -1.66E+00
PERE = Use of renewable primary energy excluding renewable primary energy resources used as raw materials; PERM = Use of renewable primary
energy resources used as raw materials; PERT = Total use of renewable primary energy resources; PENRE = Use of non-renewable primary energy
excluding non-renewable primary energy resources used as raw materials; PENRM = Use of non-renewable primary energy resources used as raw
materials; PENRT = Total use of non-renewable primary energy resources; SM = Use of secondary material; RSF = Use of renewable secondary fuels;
NRSF = Use of non-renewable secondary fuels; FW = Use of net fresh water
RESULTS OF THE LCA – WASTE CATEGORIES AND OUTPUT FLOWS according to EN 15804+A2:
1 piece Folding Door 50 / 50E
Parameter Unit A1-A3 A4 A5 B6 C1 C2 C3 C4 D
HWD kg 2.35E-05 2.57E-09 4.05E-08 0 0 1.23E-09 5.89E-08 2.88E-07 -2.29E-05
NHWD kg 5.94E+01 3E-03 2.38E+00 0 0 1E-03 3.46E+00 9.49E+01 -2.2E+01
RWD kg 2.07E-01 2.84E-05 3.98E-04 0 0 1.36E-05 5.76E-04 2.15E-04 -1.58E-01
CRU kg 0 0 0 0 0 0 0 0 0
MFR kg 0 0 0 0 0 0 5.65E+01 0 0
MER kg 0 0 0 0 0 0 0 0 0
EEE MJ 0 0 4.28E+01 0 0 0 6.2E+01 0 0
EET MJ 0 0 9.81E+01 0 0 0 1.42E+02 0 0
4 Environmental Product Declaration - KONE - Folding door system 50 / 50E
HWD = Hazardous waste disposed; NHWD = Non-hazardous waste disposed; RWD = Radioactive waste disposed; CRU = Components for re-use;
MFR = Materials for recycling; MER = Materials for energy recovery; EEE = Exported electrical energy; EET = Exported thermal energy
RESULTS OF THE LCA – additional impact categories according to EN 15804+A2-optional:
1 piece Folding Door 50 / 50E
Parameter Unit A1-A3 A4 A5 B6 C1 C2 C3 C4 D
Disease
PM 2.25E-05 9.81E-09 5.23E-08 0 0 4.7E-09 7.58E-08 1.28E-07 -9.14E-06
incidence
IR kBq U235 eq 3.26E+01 4E-03 3.6E-02 0 0 2E-03 5.2E-02 2.2E-02 -2.99E+01
ETP-fw CTUe 5.35E+03 1.87E+01 4.02E+00 0 0 8.98E+00 5.81E+00 1.08E+01 -7.63E+02
HTP-c CTUh 1.9E-05 3.53E-10 3.48E-10 0 0 1.69E-10 5.03E-10 1.6E-09 -7.25E-08
HTP-nc CTUh 6.75E-06 1.51E-08 3.51E-08 0 0 7.22E-09 5.08E-08 1.76E-07 1.64E-06
SQP SQP 7.19E+02 6.8E-02 3.2E+00 0 0 3.3E-02 4.64E+00 3.93E+00 -1.58E+02
PM = Potential incidence of disease due to PM emissions; IR = Potential Human exposure efficiency relative to U235; ETP-fw = Potential comparative
Toxic Unit for ecosystems; HTP-c = Potential comparative Toxic Unit for humans (cancerogenic); HTP-nc = Potential comparative Toxic Unit for humans
(not cancerogenic); SQP = Potential soil quality index
Disclaimer 1 – for the indicator “Potential Human exposure efficiency relative to U235”. This impact category deals mainly with the
eventual impact of low-dose ionizing radiation on human health of the nuclear fuel cycle. It does not consider effects due to possible
nuclear accidents, occupational exposure or radioactive waste disposal in underground facilities. Potential ionizing radiation from the
soil, radon and from some construction materials is also not measured by this indicator.
Disclaimer 2 – for the indicators “abiotic depletion potential for non-fossil resources”, “abiotic depletion potential for fossil resources”,
“water (user) deprivation potential, deprivation-weighted water consumption”, “potential comparative toxic unit for ecosystems”,
“potential comparative toxic unit for humans – cancerogenic”, “Potential comparative toxic unit for humans - not cancerogenic”,
“potential soil quality index”. The results of this environmental impact indicator shall be used with care as the uncertainties on these
results are high as there is limited experience with the indicator.
This EPD was created using a software tool.
References
EN 18650 Machinery Directive
EN 18650-1:2010, Powered pedestrian doors Part 1: Directive 2006/42/EC of the European Parliament and of the
Product requirements and test methods Council on machinery, and amending Directive 95/16/EC
EN 18650 Further References
EN 18650-2:2010, Powered pedestrian doors Part 2:
Safety at powered pedestrian doors IBU 2021
General Instructions for the EPD programme of Institut Bauen
EN 16005 und Umwelt e.V. Version 2.0, Berlin: Institut Bauen und Umwelt
EN 16005: 2013-01, Power operated pedestrian doorsets - e.V., 2021. www.ibu-epd.com
Safety in use Requirements and test methods
GaBi
EN 60335 Sphera Solutions GmbH Gabi Software System and Database
EN 60335-1, 2103:2020-08, Household and similar electrical for Life Cycle Engineering 1992-2020 Version 10.0.0.71
appliances - Safety - Part 1: General requirements University of Stuttgart Leinfelden Echterdingen
EN 61000 GaBi ts documentation
EN 61000-1-2: 2017-07, Electromagnetic compatibility (EMC) GaBi life cycle inventory data documentation
Part 1-2: General - Methodology for the achievement of (https://www.gabisoftware.
functional safety of electrical and electronic systems including com/support/gabi/gabidatabase 2020lcidocumentation/)
equipment with regard to electromagnetic phenomena
LCA-tool dormakaba
ISO 13849 LCA tool, ENS doors Tool No.: IBU-DOR-202108-LT1-EN
DIN EN ISO 13849-1:2021-08, Safety of machinery - Safety- Developed by Sphera Solutions GmbH
related parts of control systems - Part 1:
General principles for design PCR Part A
PCR – Part A: Calculation Rules for the Life Cycle Assessment
REACH and Requirements on the Project Report according to EN
Registration, Evaluation, Authorisation and Restriction of 15804+A2:2019, Version 1.0, Institut Bauen und Umwelt e.V.,
Chemicals (REACH), Regulation (EC) No 1907/2006 www.ibu-epd.com.
2011/65/EU ROHS3 Directive PCR Part B
Directive 2011/65/EU of the European Parliament and of the PCR – Part B: Requirements on the EPD for Automatic doors,
Council of 8 June 2011 on the restriction of the use of certain automatic gates, and revolving door systems, 08.2021, Institut
hazardous substances in electrical and electronic equipment Bauen undUmwelt e.V., www.ibu-epd.com.
5 Environmental Product Declaration - KONE - Folding door system 50 / 50E
Publisher
Institut Bauen und Umwelt e.V. +49 (0)30 3087748- 0
Hegelplatz 1 info@ibu-epd.com
10117 Berlin www.ibu-epd.com
Germany
Programme holder
Institut Bauen und Umwelt e.V. +49 (0)30 3087748- 0
Hegelplatz 1 info@ibu-epd.com
10117 Berlin www.ibu-epd.com
Germany
Author of the Life Cycle Assessment
dormakaba International Holding GmbH +49 2333 793-0
DORMA Platz 1 info.de@dormakaba.com
58256 Ennepetal www.dormakaba.com
Germany
Owner of the Declaration
KONE Corporation +358(0)204 75 1
Keilasatama 3 contact@kone.com
02150 ESPOO www.kone.com
Finland
6 Environmental Product Declaration - KONE - Folding door system 50 / 50E
