ENVIRONMENTAL PRODUCT DECLARATION
as per ISO 14025 and EN 15804+A2
Owner of the Declaration Vebe Floorcoverings B. V.
Programme holder Institut Bauen und Umwelt e.V. (IBU)
Publisher Institut Bauen und Umwelt e.V. (IBU)
Declaration number EPD-VEB-20220241-CBB1-EN
Issue date 30.11.2022
Valid to 29.11.2027
Needled carpet tiles
with a maximum pile weight of 1850 g/m2, and a pile
composition of 80% polypropylene and 20% polyester,
bitumen heavy backing
Vebe Floorcoverings B. V.
www.ibu-epd.com | https://epd-online.com
Umwelt Produktdeklaration Name des Herstellers – Name des Produkts
General Information
Vebe Floorcoverings B.V. Needled carpet tiles
with a maximum pile weight of 1850
g/m2 and a pile composition of 80%
polypropylene and 20% polyester,
bitumen heavy backing
Programme holder Owner of the declaration
IBU – Institut Bauen und Umwelt e.V. Vebe Floorcoverings B.V.
Hegelplatz 1 Inslag 12
10117 Berlin 8281 JV, Genemuiden
Germany Netherlands
www.vebe.eu
Declaration number Declared product / declared unit
EPD-VEB-20220241-CBB1-EN 1 m² needled tiles, PP and PET pile material with a
bitumen heavy backing
This declaration is based on the product Scope:
category rules: The manufacturer declaration applies to a group of
Floor coverings, 02.2018 needled carpet tiles with a bitumen heavy backing, The
(PCR checked and approved by the SVR) pile material consists of minimum 80% polypropylene
and maximum 20% of polyester. The maximum total
pile weight is 1850 g/m2. The products are needled and
Issue date
cut in Genemuiden, Netherlands and the bitumen
30.11.2022
backing is applied in Nijkerk, Netherlands.
LCA results for products with a maximum total pile
Valid to
weight of 750 g/m2 can be taken from the
29.11.2027 corresponding tables of the annexe. Specific data for
every product within the declared group of products in
relation to its total pile weight can be calculated by
using equation 1 given in the annexe (see annexe
chapter: 'General Information on the annexe'). The
declaration is only valid in conjunction with a valid
GUT-PRODIS license of the product.
The owner of the declaration shall be liable for the
underlying information and evidence; the IBU shall not
be liable with respect to manufacturer information, life
cycle assessment data and evidences.
The EPD was created according to the specifications
of EN 15804+A2. In the following, the standard will be
simplified as EN 15804.
Verification
The standard EN 15804 serves as the core PCR
Independent verification of the declaration and data
according to ISO 14025:2011
Dipl. Ing. Hans Peters internally x externally
(chairman of Institut Bauen und Umwelt e.V.)
Dr. Alexander Röder Angela Schindler
(Managing Director Institut Bauen und Umwelt e.V.)) (Independent verifier)
Product
Product description/Product definition carpet is 8% having 20% polyester in the pile material
The declaration applies to needled carpet tiles with a and a maximum total pile weight of 1850g/m2.
bitumen heavy backing. The pile material consists of at
least 80% Polypropylene and max. 20% of polyester For the placing on the market of the specific product in
which is 100% recycled. Maximum total pile weight is the European Union/European Free Trade Association
1850 g/m2. The maximum recycled content of the (EU/EFTA) (with the exception of Switzerland)
Regulation (EU) No. 305/2011 Construction Product
2 Environmental Product Declaration Vebe Floorcoverings B. V. – Needled carpet tiles, yarn mixture of 80% polypropylene,
20% polyester and a bitumen heavy backing
Regulation (CPR) applies. The product needs a Base materials/Ancillary materials
Declaration of Performance (DoP) taking into
consideration EN 14041:2018-05, Resilient, textile and Name Value Unit
laminate floor coverings - Essential characteristics, and Polypropylene 29,2 %
the CE-marking. The DoP of the product can be found Polyester 8,2 %
on the manufacturer's technical information section. SBR Latex 6,8 %
For the application and use of the product the Bitumen 16,6 %
respective national provisions apply. Limestone 38,8 %
Glass fiber 0,2 %
Application Additives 0,2 %
The use class of the specific product as defined in
EN 1307 can be found in the Product Information
The specific product coverd by the EPD contains
System (PRODIS) using the PRODIS registration
substances listed in the ECHA candidate list
number of the product.
(08.07.2021) or other carcinogenic, mutagenic or
reprotoxic (CMR) substances in categories 1A or 1B
Technical Data
which are not on the candidate list exceeding 0.1
The technical data describes a fictitious worst-case
percentage by mass: no
product representing all products with the described
The products are registered in the GUT-PRODIS
characteristics.
Information System. The PRODIS system ensures the
compliance with limitations of various chemicals and
Constructional data according to EN 1307
Volatile Organic Compound (VOC)-emissions and a
Name Value Unit ban on the use of all substances that are listed as
Product Form Tiles -
'Substances of Very High Concern' (SVHC) under
Type of manufacture Needled carpet -
REACH.
Yarn type 80% PP / 20% PET -
Total carpet weight 5065 g/m2 Reference service life
bitumen heavy The service life of textile floor coverings strongly
Secondary backing -
backing depends on the correct installation taking into account
the declared use classification and the adherence to
cleaning and maintenance instructions.
Performance data of the product in accordance with A calculation of the reference service life according to
the declaration of performance with respect to its ISO 15686 is not possible.
essential characteristics according to EN 14041: 2018- Alternatively, a reference service life of 10 years can
05, Resilient, textile and laminate floor coverings - be assumed, during which the functional and visual
Essential characteristics. quality is guaranteed (BNB, Nutzungsdauer von
Additional product properties in accordance with EN Bauteilen). The technical service life can be
1307 can be found on the Product Information System significantly longer.
PRODIS using the PRODIS registration number of the
product (www.pro-dis.info) or on the manufacturer's
technical information section.
LCA: Calculation rules
Declared Unit System boundaries of modules A, B, C, D:
Modules C3, C4 and D are indicated separately for
three end-of-life scenarios:
Name Value Unit 1 - landfill disposal
Declared unit 1 m2 2 - municipal waste incineration
Grammage 5065 kg/m2 3 - recovery in a cement plant
The declared unit refers to 1 m2 produced textile floor
covering. The Output of module A5 'Assembly' is 1 m2 A1-A3 Production:
installed textile floor covering. Energy supply and production of the basic material,
The layer thickness of the specific product covered by processing of secondary material, auxiliary material,
the EPD can be found on the Product Information transport of the material to the manufacturing site,
System PRODIS using the PRODIS registration emissions, waste water treatment, packaging material
number of the product (www.pro-dis.info) or on the and waste processing up to the landfill disposal of
manufacturer's technical information section. residual waste (except radioactive waste). Benefits for
generated electricity and steam due to the incineration
of production waste are aggregated.
Biogenic carbon that is stored in renewable material
System boundary (packaging paper) is taken into account as well as the
associated carbon dioxide uptake from the air from
Type of EPD: Cradle-to-grave which this biogenic carbon comes.
3 Environmental Product Declaration Vebe Floorcoverings B. V. – Needled carpet tiles, yarn mixture of 80% polypropylene,
20% polyester and a bitumen heavy backing
The floor covering is de-constructed manually and no
A4 Transport: additional environmental impact is caused.
Transport of the packed textile floor covering
from factory gate to the place of installation. C2 Transport:
Transport of the carpet waste to a landfill, to the
A5 Installation: municipal waste incineration plant (MWI) or to the
Installation of the textile floor covering, processing of waste collection facility for recycling.
installation waste and packaging waste up to the
landfill disposal of residual waste (except radioactive C3 Waste processing:
waste), the production of the amount of carpet that C3-1: Landfill disposal needs no waste processing.
occurs as installation waste including its transport to C3-2: Impact from waste incineration (plant with
the place of installation. R1>0.6), generated electricity and steam are listed in
Generated electricity and steam due to the incineration the result table as exported energy.
of waste are listed in the result table as exported C3-3: Collection of the carpet waste for recovery in the
energy. cement industry, waste processing (granulating),
Biogenic carbon that is stored in renewable materials transport to the cement plant, emissions from the
in packaging paper is released as carbon dioxide incineration.
emissions into the air at the end of life in module A5.
Preparation of the floor and auxiliary materials C4 Disposal
(adhesives, fixing agents, PET connectors) are beyond C4-1: Impact from landfill disposal,
the system boundaries and not taken into account. C4-2: The carpet waste leaves the system in
module C3-2,
B1 Use: C4-3: The pre-processed carpet waste leaves the
Indoor emissions during the use stage. After the first system in module C3-3.
year, no product-related Volatile Organic Compound
(VOC) emissions are relevant due to known VOC D Recycling potential:
decay curves of the product. Calculated benefits result from materials exclusive
secondary materials (net materials).
B2 Maintenance: D-A5: Benefits for generated energy due
Cleaning of the textile floor covering for a period of 1 to incineration of packaging and installation waste
year: (incineration plant with R1 > 0.6),
Vacuum cleaning – electricity supply D-1: Benefits for generated energy due to landfill
Wet cleaning – electricity, water consumption, disposal of carpet waste at the end-of-life,
production of the cleaning agent, waste water D-2: Benefits for generated energy due to incineration
treatment. of carpet waste at the end-of-life (incineration plant
The declared values in this module have to be with R1 > 0.6),
multiplied by the assumed service life of the floor D-3: Benefits for saved fossil energy and saved
covering in the building in question. inorganic material due to recovery of the carpet in a
cement plant.
B3 - B5:
The modules are not relevant within the assumed Comparability
reference service life of 10 years. Basically, a comparison or an evaluation of EPD data
is only possible if all the data sets to be compared
B6 - B7: were created according to EN 15804 and the building
No energy and water input are required for the context, respectively the product-specific
operation of the carpet in the use stage. The modules characteristics of performance, are taken into account.
do not cause any environmental impact.
Background data are taken from the GaBi database,
C1 De-construction: 2021-2. Remaining data gaps are covered by the
ecoinvent 3.7 database, 2020.
LCA: Scenarios and additional technical information
Characteristic product properties Capacity utilisation (including
55 %
Information on biogenic Carbon empty runs)
Installation in the building (A5)
Name Value Unit Name Value Unit
Biogenic Carbon Content in Material loss 0.152 kg
accompanying packaging at 0.001 kg C Polyethylene packaging waste and installation waste
factory gate are considered to be incinerated in a municipal waste
1 kg biogenic Carbon is equivalent to 44/12 kg of CO 2 incineration plant. Cardboard packaging waste is going
to be recycled.
Preparation of the floor and auxiliaries (adhesives,
fixing agents, PET connectors etc.) are not taken into
Transport to the construction site (A4) account.
Name Value Unit
Litres of fuel (truck, EURO 0-6 Maintenance (B2)
0.0119 l/100km
mix) The values for cleaning refer to 1 m2 floor covering per
Transport distance 700 km year.
4 Environmental Product Declaration Vebe Floorcoverings B. V. – Needled carpet tiles, yarn mixture of 80% polypropylene,
20% polyester and a bitumen heavy backing
Depending on the application based on ISO 10874, the
technical service life recommended by the Recycling in the cement industry (scenario 3)
manufacturer and the anticipated strain on the floor by The organic material of the carpet is used as an
customers, the case-specific useful life can be alternative fuel in a cement kiln. It mainly substitutes
established. Based on this useful life the effects of for lignite (68.8 %), hard coal (23.6 %) and petrol coke
module B2 need to be calculated in order to obtain the (7.6 %). The inorganic material is substantially
overall environmental impacts. integrated into the cement clinker and substitutes for
original material input. VDZ e.V.
Name Value Unit
Maintenance cycle (vacuum Number
208
cleaning) /year
Number
Maintenance cycle (wet cleaning) 1,5
/year
Water consumption (wet cleaning) 0.004 m3
Cleaning agent (wet cleaning) 0.09 kg
Electricity consumption 0.314 kWh
For further information on cleaning and maintenance
see www.vebe.eu
Service life
Name Value Unit
Life Span (according to BBSR) 10 a
Corresponds to
Declared product properties (at the
-
the gate) and finishes specifications of
EN 1307
An assumed quality of work, when Conforms to the
installed in accordance with the manufacturer's -
manufacturer’s instructions instructions
Use in areas
defined by the
Usage conditions, e.g. frequency
use class -
of use, mechanical exposure
according to EN
1307
Maintenance e.g. required According to the
frequency, type and quality and manufacturers -
replacement of components instructions
End of Life (C1-C4)
Three different end-of-life scenarios are declared and
the results are indicated separately in module C.
Each scenario is calculated as a 100% scenario.
Scenario 1: 100 % landfill disposal
Scenario 2: 100 % municipal waste incineration (MWI)
with R1>0.6
Scenario 3: 100 % recovery in the cement industry
If combinations of these scenarios have to be
calculated this should be done according to the
following scheme:
EOL-impact = x % impact (Scenario 1)
+ y % impact (Scenario 2)
+ z % impact (Scenario 3)
with x % + y % + z % = 100 %
Name Value Unit
Collected as mixed construction
5.065 kg
waste (scenario 1 and 2)
Collected separately (scenario 3) 5.065 kg
Landfilling (scenario 1) 5.065 kg
Energy recovery (scenario 2) 5.065 kg
Energy recovery (scenario 3) 3,088 kg
Recycling (scenario 3) 1.977 kg
Reuse, recovery and/or recycling potentials (D),
relevant scenario information
Recovery or recycling potentials due to the three end-
of-life scenarios (module C) are indicated separately.
5 Environmental Product Declaration Vebe Floorcoverings B. V. – Needled carpet tiles, yarn mixture of 80% polypropylene,
20% polyester and a bitumen heavy backing
LCA: Results
The LCA results refer to all declared products with a maximum total pile weight of 1850 g/m2. LCA results for
products with a maximum total pile weight of 750 g/m2 can be taken from the corresponding tables of the annexe.
Results for specific products with any other total pile weight can be calculated by using equation 1 given in the
annexe (see annexe chapter: 'General Information on the annexe'). The declared result figures in module B2 have
to be multiplied by the assumed service life (in years) of the floor covering in the building under consideration.
Information on non-relevant modules: Modules B3 - B7 are not relevant during the service life of the carpet.
Modules C1, C3/1, C4/2 and C4/3 cause no additional impact (see chapter "LCA: Calculation rules" in this
document). All these modules are declared and marked as 'modules not relevant/declared'. Module C2 represents
the transport for scenarios 1, 2 and 3. Column D represents module D/A5.
DESCRIPTION OF THE SYSTEM BOUNDARY (X = INCLUDED IN LCA; ND = MODULE OR INDICATOR NOT
DECLARED; MNR = MODULE NOT RELEVANT)
BENEFITS AND
CONSTRUCTI LOADS
PRODUCT STAGE ON PROCESS USE STAGE END OF LIFE STAGE BEYOND THE
STAGE SYSTEM
BOUNDARIES
6 Environmental Product Declaration Vebe Floorcoverings B. V. – Needled carpet tiles, yarn mixture of 80% polypropylene,
20% polyester and a bitumen heavy backing
lairetam
waR
ylppus tropsnarT
gnirutcafunaM
eht
morf
tropsnarT
etis
eht
ot
etag
ylbmessA esU
ecnanetniaM
riapeR
tnemecalpeR tnemhsibrufeR
ygrene
lanoitarepO esu
retaw
lanoitarepO esu
noitcurtsnoc-eD
noitilomed tropsnarT
gnissecorp
etsaW
lasopsiD -esueR -yrevoceR -gnilcyceR laitnetop
A1 A2 A3 A4 A5 B1 B2 B3 B4 B5 B6 B7 C1 C2 C3 C4 D
X X X X X X X MNR MNR MNR ND ND X X X X X
RESULTS OF THE LCA - ENVIRONMENTAL IMPACT according to EN 15804+A2: 1 m² floor covering
Core Indicator Unit A1-A3 A4 A5 B1 B2 C1 C2 C3/2 C3/3 C4/1 D D/1 D/2 D/3
-
GWP-total [kg CO2-Eq.] 6.91E+03.01E-1 4.66E-10.00E+04.16E-10.00E+01.72E-28.06E+08.13E+03.55E-1-7.61E-20.00E+0 2.49E+0-5.86E-1
-
GWP-fossil [kg CO2-Eq.] 6.90E+02.96E-1 4.61E-10.00E+02.15E-10.00E+01.69E-28.06E+08.13E+03.55E-1-7.57E-20.00E+0 2.48E+0-5.85E-1
GWP-biogenic [kg CO2-Eq.] 6.78E-3 3.83E-3 5.34E-30.00E+04.16E-30.00E+02.18E-4 5.95E-4 1.38E-30.00E+0-3.85E-40.00E+0-1.26E-2-3.74E-4
GWP-luluc [kg CO2-Eq.] 5.67E-3 1.67E-3 2.30E-40.00E+01.96E-10.00E+09.56E-5 2.15E-4 4.60E-4 1.75E-4-8.27E-60.00E+0-2.71E-4-2.62E-4
1.80E- 1.57E- 1.03E- 5.04E- 8.86E- 4.82E- -5.08E- -1.66E- -1.14E-
ODP [kg CFC11-Eq.] 5.23E-9 0.00E+03.42E-80.00E+0 0.00E+0
14 10 15 13 13 13 13 11 12
AP [mol H+-Eq.] 1.70E-2 1.79E-3 6.17E-40.00E+08.32E-40.00E+01.02E-4 1.73E-3 2.04E-3 1.06E-3-9.91E-50.00E+0-3.25E-3-1.71E-3
EP-freshwater [kg P-Eq.] 2.43E-5 8.96E-7 7.82E-70.00E+05.19E-60.00E+05.12E-8 7.86E-7 9.90E-7 6.70E-5-1.03E-70.00E+0-3.39E-6-6.45E-7
EP-marine [kg N-Eq.] 4.59E-3 8.78E-4 1.83E-40.00E+01.97E-40.00E+05.01E-5 5.87E-4 7.25E-4 2.35E-4-2.69E-50.00E+0-8.83E-4-5.85E-4
EP-terrestrial [mol N-Eq.] 4.89E-2 9.71E-3 2.01E-30.00E+02.83E-30.00E+05.55E-4 7.80E-3 9.32E-3 2.58E-3-2.89E-40.00E+0-9.46E-3-6.41E-3
POCP [kg NMVOC-Eq.]1.49E-2 1.66E-3 5.46E-4 4.18E-4 9.83E-40.00E+09.47E-5 1.58E-3 1.85E-3 7.57E-4-7.54E-50.00E+0-2.47E-3-1.81E-3
ADPE [kg Sb-Eq.] 1.19E-6 2.51E-8 3.72E-80.00E+02.30E-70.00E+01.43E-9 2.44E-8 3.51E-8 2.49E-8-1.14E-80.00E+0-3.72E-7-5.41E-8
- - -
ADPF [MJ] 2.26E+24.01E+06.97E+00.00E+05.90E+00.00E+02.29E-12.66E+03.71E+05.09E+0 0.00E+0
1.29E+0 4.22E+19.38E+1
[m³ world-Eq
WDP 1.04E+12.69E-3 3.40E-10.00E+09.99E-20.00E+01.53E-4 9.31E-1 9.37E-1-3.81E-3-7.91E-30.00E+0-2.59E-1-9.38E-2
deprived]
GWP = Global warming potential; ODP = Depletion potential of the stratospheric ozone layer; AP = Acidification potential of land and water; EP =
Caption Eutrophication potential; POCP = Formation potential of tropospheric ozone photochemical oxidants; ADPE = Abiotic depletion potential for non-
fossil resources; ADPF = Abiotic depletion potential for fossil resources; WDP = Water (user) deprivation potential
RESULTS OF THE LCA - INDICATORS TO DESCRIBE RESOURCE USE according to EN 15804+A2: 1 m²
floor covering
Indicator Unit A1-A3 A4 A5 B1 B2 C1 C2 C3/2 C3/3 C4/1 D D/1 D/2 D/3
PERE [MJ] 1.88E+1 2.28E-1 5.96E-1 0.00E+0 3.69E+0 0.00E+0 1.30E-2 5.43E-1 8.37E-1 4.19E-1 -3.51E-1 0.00E+0 -1.15E+1-6.84E-1
PERM [MJ] 7.00E-3 0.00E+0 -7.00E-3 0.00E+0 0.00E+0 0.00E+0 0.00E+0 0.00E+0 0.00E+0 0.00E+0 0.00E+0 0.00E+0 0.00E+0 0.00E+0
PERT [MJ] 1.89E+1 2.28E-1 5.89E-1 0.00E+0 3.69E+0 0.00E+0 1.30E-2 5.43E-1 8.37E-1 4.19E-1 -3.51E-1 0.00E+0 -1.15E+1-6.84E-1
PENRE [MJ] 1.20E+2 4.02E+0 7.02E+0 0.00E+0 5.90E+0 0.00E+0 2.30E-1 1.09E+2 1.10E+2 5.10E+0 -1.29E+0 0.00E+0 -4.22E+1-9.38E+1
PENRM [MJ] 1.06E+2 0.00E+0 -3.70E-2 0.00E+0 0.00E+0 0.00E+0 0.00E+0 -1.06E+2-1.06E+2 0.00E+0 0.00E+0 0.00E+0 0.00E+0 0.00E+0
PENRT [MJ] 2.26E+2 4.02E+0 6.98E+0 0.00E+0 5.90E+0 0.00E+0 2.30E-1 2.66E+0 3.71E+0 5.10E+0 -1.29E+0 0.00E+0 -4.22E+1-9.38E+1
SM [kg] 3.86E-1 0.00E+0 1.16E-2 0.00E+0 0.00E+0 0.00E+0 0.00E+0 0.00E+0 0.00E+0 0.00E+0 0.00E+0 0.00E+0 0.00E+0 1.11E+0
RSF [MJ] 0.00E+0 0.00E+0 0.00E+0 0.00E+0 0.00E+0 0.00E+0 0.00E+0 0.00E+0 0.00E+0 0.00E+0 0.00E+0 0.00E+0 0.00E+0 0.00E+0
NRSF [MJ] 0.00E+0 0.00E+0 0.00E+0 0.00E+0 0.00E+0 0.00E+0 0.00E+0 0.00E+0 0.00E+0 0.00E+0 0.00E+0 0.00E+0 0.00E+0 0.00E+0
FW [m³] 2.52E-1 2.58E-4 8.24E-3 0.00E+0 3.34E-3 0.00E+0 1.47E-5 2.19E-2 2.22E-2 5.97E-5 -3.35E-4 0.00E+0 -1.10E-2 -8.16E-3
PERE = Use of renewable primary energy excluding renewable primary energy resources used as raw materials; PERM = Use of
renewable primary energy resources used as raw materials; PERT = Total use of renewable primary energy resources; PENRE = Use of
non-renewable primary energy excluding non-renewable primary energy resources used as raw materials; PENRM = Use of non-
Caption
renewable primary energy resources used as raw materials; PENRT = Total use of non-renewable primary energy resources; SM = Use
of secondary material; RSF = Use of renewable secondary fuels; NRSF = Use of non-renewable secondary fuels; FW = Use of net fresh
water
RESULTS OF THE LCA – WASTE CATEGORIES AND OUTPUT FLOWS according to EN 15804+A2:
1 m² floor covering
Indicator Unit A1-A3 A4 A5 B1 B2 C1 C2 C3/2 C3/3 C4/1 D D/1 D/2 D/3
HWD [kg] 9.19E-6 1.93E-11 2.76E-7 0.00E+0 4.19E-5 0.00E+0 1.10E-123.29E-103.72E-107.86E-10-1.75E-100.00E+0 -5.73E-9-1.63E-10
NHWD [kg] 1.05E-1 5.76E-4 3.68E-2 0.00E+0 7.30E-3 0.00E+0 3.29E-5 1.12E+0 1.12E+0 5.04E+0 -6.48E-4 0.00E+0 -2.12E-2 -1.87E-3
RWD [kg] 7.89E-3 4.95E-6 2.41E-4 0.00E+0 3.76E-4 0.00E+0 2.83E-7 1.24E-4 2.00E-4 6.26E-5 -1.01E-4 0.00E+0 -3.30E-3 -1.32E-4
CRU [kg] 0.00E+0 0.00E+0 0.00E+0 0.00E+0 0.00E+0 0.00E+0 0.00E+0 0.00E+0 0.00E+0 0.00E+0 0.00E+0 0.00E+0 0.00E+0 0.00E+0
MFR [kg] 0.00E+0 0.00E+0 3.40E-3 0.00E+0 0.00E+0 0.00E+0 0.00E+0 0.00E+0 1.11E+0 0.00E+0 0.00E+0 0.00E+0 0.00E+0 0.00E+0
MER [kg] 0.00E+0 0.00E+0 0.00E+0 0.00E+0 0.00E+0 0.00E+0 0.00E+0 0.00E+0 0.00E+0 0.00E+0 0.00E+0 0.00E+0 0.00E+0 0.00E+0
EEE [MJ] 0.00E+0 0.00E+0 3.74E-1 0.00E+0 0.00E+0 0.00E+0 0.00E+0 1.23E+1 0.00E+0 0.00E+0 0.00E+0 0.00E+0 0.00E+0 0.00E+0
EET [MJ] 0.00E+0 0.00E+0 6.82E-1 0.00E+0 0.00E+0 0.00E+0 0.00E+0 2.24E+1 1.15E+2 0.00E+0 0.00E+0 0.00E+0 0.00E+0 0.00E+0
HWD = Hazardous waste disposed; NHWD = Non-hazardous waste disposed; RWD = Radioactive waste disposed; CRU = Components
Caption for re-use; MFR = Materials for recycling; MER = Materials for energy recovery; EEE = Exported electrical energy; EET = Exported
thermal energy
RESULTS OF THE LCA – additional impact categories according to EN 15804+A2-optional:
1 m² floor covering
Indicator Unit A1-A3 A4 A5 B1 B2 C1 C2 C3/2 C3/3 C4/1 D D/1 D/2 D/3
[Disease -8.21E-
PM 1.77E-7 1.03E-8 6.15E-9 0.00E+0 6.84E-8 0.00E+05.90E-10 1.72E-8 1.91E-8 1.02E-8 0.00E+0 0.00E+0 -3.73E-8
Incidence] 10
[kBq U235-
IRP 8.65E-1 7.26E-4 2.66E-2 0.00E+0 6.78E-2 0.00E+0 4.14E-5 1.93E-2 3.22E-2 9.24E-3 -1.70E-2 0.00E+0 0.00E+0 -1.14E-2
Eq.]
ETP-fw [CTUe] 1.29E+2 2.79E+0 4.01E+0 3.60E-3 2.69E+0 0.00E+0 1.59E-1 1.59E+0 2.19E+0 4.99E+0 -2.80E-1 0.00E+0 0.00E+0-1.58E+1
-1.30E- -1.41E-
HTP-c [CTUh] 2.87E-9 5.63E-119.07E-110.00E+06.21E-100.00E+03.21E-129.34E-111.07E-102.24E-10 0.00E+0 0.00E+0
11 10
-4.98E-
HTP-nc [CTUh] 1.50E-7 3.34E-9 4.79E-9 2.60E-11 9.46E-9 0.00E+01.91E-10 6.13E-9 6.82E-9 1.88E-8 0.00E+0 0.00E+0 -7.26E-9
10
SQP [-] ND ND ND ND ND 0.00E+0 ND ND ND ND ND ND ND ND
PM = Potential incidence of disease due to PM emissions; IR = Potential Human exposure efficiency relative to U235; ETP-fw = Potential
Caption comparative Toxic Unit for ecosystems; HTP-c = Potential comparative Toxic Unit for humans (cancerogenic); HTP-nc = Potential
comparative Toxic Unit for humans (not cancerogenic); SQP = Potential soil quality index
No substantiated values can be given for the SQP indicator with the existing database.
The result figures given in module B2 refer to a period of 1 year because a reference service life is not declared.
They have to be multiplied by the assumed service life (in years) of the floor covering in the building under
consideration.
Disclaimer 1 – for the indicator “Potential Human exposure efficiency relative to U235”.
This impact category deals mainly with the eventual impact of low dose ionizingradiation on human health of the
nuclear fuel cycle. It does not consider effects due to possible nuclear accidents, occupational exposure or to
radioactive waste disposal in undergroundfacilities. Potential ionizing radiation from the soil, radon and from some
construction materials is also not measured by this indicator.
Disclaimer 2 – for the indicators “abiotic depletion potential for non-fossil resources”, “abiotic depletion potential
for fossil resources”, “water (user) deprivation potential, deprivation-weighted water consumption”, “potential
comparative toxic unit for ecosystems”, “potential comparative toxic unit for humans – cancerogenic”, “Potential
comparative toxic unit for humans - not cancerogenic”, “potential soil quality index”.
The results of this environmental impact indicator shall be used with care as the uncertainties on these results are
high as there is limited experience with the indicator.
References
EN 1307 floor coverings – Environmental product declarations –
DIN EN 1307: 2014+A1:2016+A2:2018-05: Textile Product category rules
floor coverings - Classification
ISO 10874
EN 13501-1 DIN EN ISO 10874: 2012+A1:2021-04: Resilient,
DIN EN 13501-1:2019-05: Fire classification of textile and laminate floor coverings - Classification
construction products and building elements - Part 1:
Classification using data from reaction to fire tests ISO 14025
DIN EN /ISO 14025:2011-10/, Environmental labels
EN 14041 and declarations — Type III environmental
DIN EN 14041: 2018-05 and DIN EN 14041: 2008-05: declarations — Principles and procedures
Resilient, textile and laminate floor coverings -
Essential characteristics
ISO 14040
EN 15804 DIN EN ISO 14040:2006+A1:2020 Environmental
DIN EN 15804:2012+A2:2019 + AC:2021, management - Life cycle assessment - Principles and
Sustainability of construction works — Environmental framework
Product Declarations — Core rules for the product
category of construction products ISO 14044
DIN EN ISO 14044:2006+A1:2018+A2:2020
EN 16810 Environmental management - Life cycle assessment -
DIN EN 16810: 2017-08: Resilient, textile and laminate Requirements and guidelines
7 Environmental Product Declaration Vebe Floorcoverings B. V. – Needled carpet tiles, yarn mixture of 80% polypropylene,
20% polyester and a bitumen heavy backing
ISO 15686 GaBi database
ISO 15686: Buildings and constructed assets - GaBi Software-System and Database for Life Cycle
Service life planning Engineering, thinkstep AG, Leinfelden-Echterdingen,
ISO 15686-1: 2011-05: Part 1: General principles and 2022-1
framework
ISO 15686-2: 2012-05: Part 2: Service life prediction PCR Part A
procedures Product Category Rules for Building-Related Products
ISO 15686-7: 2017-04: Part 7: Performance and Services Part A: Calculation Rules for the Life
evaluation for feedback of service life data Cycle Assessment and Requirements on the Project
from practice Report according to EN 15804+A2:2019, V1.1, Berlin:
ISO 15686-8: 2008-06: Part 8: Reference service life Institut Bauen und Umwelt e.V. (IBU), January 2021
and service-life estimation
PCR Part B
Regulation (EU) No. 305/2011 Product Category Rules for Building-Related Products
Regulation No. 305/2011 Construction Products and Services
Regulation (CPR) of the European Council and of the Part B: Requirements on the EPD for floor coverings,
European Parliament, April 2011 V1.2, Berlin: Institut Bauen und Umwelt e.V. (IBU),
February 2018
General Instructions for the IBU-EPD Program
General Instructions for the EPD-Program of the PRODIS
Institut Bauen und Umwelt e.V., The Preparation of Product Information System (PRODIS) of the
Environmental Product Declarations - EPDs, version European Carpet Industry, Gemeinschaft
2.0, Institut Bauen und Umwelt e.V., Berlin, January umweltfreundlicher Teppichboden e.V (GUT) and
2021, www.ibu-epd.de European Carpet and Rug Association
(ECRA), http://www.pro-dis.info
BNB, Nutzungsdauer von Bauteilen
Bewertungssystem Nachhaltiges Bauen (BNB), REACH
Nutzungsdauer von Bauteilen, Bundesministerium des Regulation (EC) No 1907/2006 of the European
Inneren, für Bau und Heimat, 24.02.2017 Parliament and of the Council of 18 December 2006
concerning the Registration, Evaluation, Authorisation
ECHA candidate list and Restriction of Chemicals (REACH), June 2017,
Candidate List of substances of very high concern last update: 08.07.2021
(SVHCs) for authorisation, 08.07.2021, European
Chemicals Agency (ECHA), Helsinki, Finland VDZ e.V.
Association of German Cement Works, Ed. Environ-
mental Data of the German Cement Industry 2020
ecoinvent
ecoinvent, Zurich, Switzerland, database version 3.7,
published September 2020
8 Environmental Product Declaration Vebe Floorcoverings B. V. – Needled carpet tiles, yarn mixture of 80% polypropylene,
20% polyester and a bitumen heavy backing
Publisher
Institut Bauen und Umwelt e.V. Tel +49 (0)30 3087748- 0
Hegelplatz 1 Fax +49 (0)30 3087748- 29
10117 Berlin Mail info@ibu-epd.com
Germany Web www.ibu-epd.com
Programme holder
Institut Bauen und Umwelt e.V. Tel +49 (0)30 - 3087748- 0
Hegelplatz 1 Fax +49 (0)30 – 3087748 - 29
10117 Berlin Mail info@ibu-epd.com
Germany Web www.ibu-epd.com
Author of the Life Cycle
Assessment Tel +49 (0)241 96843 410
Gemeinschaft umweltfreundlicher Fax +49 (0)241 96843 400
Teppichboden (GUT) e.V. Mail mail@gut-ev.de
Schönebergstraße 2 Web www.gut-ev.org
52068 Aachen
Germany
Owner of the Declaration
Vebe Floorcoverings B.V. Tel +31 (0)38 3853200
Inslag 12 Fax +31 (0)38 3856187
8281JV Genemuiden Mail info@vebe.net
Netherlands Web www.condor-
group.eu/vebe_floorcoverings
