Environmental product declaration
in accordance with ISO 14025 and EN 15804+A2
Geniox GO (R-HW-Optimized)
Owner of the declaration: Program operator:
UAB Systemair The Norwegian EPD Foundation
Product: Declaration number:
Geniox GO (R-HW-Optimized) NEPD-8444-8104-EN
Declared unit: Registration number:
1 pcs NEPD-8444-8104-EN
This declaration is based on Product Category Rules: Issue date:
CEN Standard EN 15804:2012+A2:2019 serves as core 11.12.2024
PCR
The Norwegian EPD Foundation NPCR 030:2021 Part B for ventilation components Valid to:
11.12.2029
ver-140125
EPD software:
LCAno EPD generator ID: 589690
1 / 14
General information
Product Owner of the declaration:
Geniox GO (R-HW-Optimized) UAB Systemair
Contact person: Darius Katinas
Phone: +370 340 601 65
e-mail: info@systemair.lt
Program operator: Manufacturer:
The Norwegian EPD Foundation UAB Systemair
Post Box 5250 Majorstuen, 0303 Oslo, Norway
Phone: +47 977 22 020
web: www.epd-norge.no
Declaration number: Place of production:
NEPD-8444-8104-EN UAB Systemair
Linu g. 101
20174 Ukmerge, Lithuania
This declaration is based on Product Category Rules: Management system:
CEN Standard EN 15804:2012+A2:2019 serves as core PCR ISO 9001, ISO 14001
NPCR 030:2021 Part B for ventilation components
Statement of liability: Organisation no:
The owner of the declaration shall be liable for the underlying LT100001604716
information and evidence. EPD Norway shall not be liable with respect
to manufacturer information, life cycle assessment data and
evidences.​
Declared unit: Issue date:
1 pcs Geniox GO (R-HW-Optimized) 11.12.2024
Declared unit with option: Valid to:
A1-A3,A4,C1,C2,C3,C4,D 11.12.2029
Year of study:
2023
Functional unit: Comparability:
Not declared. EPD of construction products may not be comparable if they not
comply with EN 15804 and seen in a building context.
General information on verification of EPD from EPD tools: Development and verification of EPD:
Independent verification of data, other environmental information The declaration is created using EPD tool lca.tools ver EPD2022.03,
and the declaration according to ISO 14025:2010, § 8.1.3 and § 8.1.4. developed by LCA.no. The EPD tool is integrated in the company's
Verification of each EPD is made according to EPD-Norway’s management system and has been approved by EPD Norway.
guidelines for verification and approval requiring that tools are i) NEPDT75 Systemair AB
integrated into the company's environmental management system, ii)
the procedures for use of the EPD tool are approved by EPD-Norway, Developer of EPD: Vilius Burneika
and iii) the process is reviewed annually by an independent third
Reviewer of company-specific input data and EPD:​ Darius Katinas
party verifier. See Appendix G of EPD-Norway's General Programme
Instructions for further information on EPD tools
Verification of EPD tool: Approved:
Independent third party verification of the EPD tool, background data
and test-EPD in accordance with EPDNorway's procedures and
guidelines for verification and approval of EPD tools.
Third party verifier:
Alexander Borg, Asplan Viak AS
(no signature required)
2 / 14
Product
Product description:
Geniox air handling unit with rotary heat exchanger, integrated controls, dampers and hydronic heater. For use in ordinary comfort ventilation.
Product specification
Geniox air handling units range from size 10 to 31, with capacities from approximately 1 000 m3/h to 35 000 m3/h.
The EPD data is provided for size 18 (reference).
Materials kg %
Adhesive 2,88 0,24
Electronic - Unspecified 8,68 0,72
Filter, plastic based 0,16 0,01
Glass fibre reinforced plastic,
84,15 6,94
polyamide
Hydronic coil (50% AL, 50%CU) 28,00 2,31
Insulation, Mineral based 43,26 3,57
Metal - Galvanized Steel 105,63 8,72
Metal - Steel with magnelis coating 635,70 52,45
Motor 65,00 5,36
Plastic - Polyamide 5,23 0,43
Plastic - Polyethylene 0,11 0,01
Plastic - Polyethylene (HDPE) 0,60 0,05
Plastic - Polypropylene (PP) 1,10 0,09
Plastic - Polyvinyl chloride (PVC) 25,03 2,06
Rubber, synthetic 11,83 0,98
Metal - Aluminium 163,00 13,45
Metal - Copper 2,00 0,17
Metal - Steel 8,14 0,67
Metal - Steel with aluzinc coating 0,66 0,05
Chemical 0,32 0,03
Other 0,30 0,02
Plastic - Acrylonitrile butadiene
17,88 1,48
styrene (ABS)
Plastic - Polycarbonate (PC) 0,50 0,04
Plastics 1,75 0,14
Total 1211,91 100,00
Packaging kg %
Packaging - Paper 0,20 4,61
Packaging - Plastic 4,14 95,39
Total incl. packaging 1216,25 100,00
Technical data:
Casing performance in accordance with EN 1886:2007:
- Air leakage class L1(M)
- Thermal bridging class TB2
- Thermal transmittance class T2
- Mechanical strength class D1
ZM310 coated steel panels with 60 mm insulation. Corrosion resistance class C5 in accordance with ISO 12944-2:2017.
Energy performance must be calculated using realistic project specific operating conditions. Complete and project specific product specification
including all relevant technical data and energy performance can be generated using our AHU calculation software, SystemairCAD. Please refer to
the Systemair website for more information.
Geniox is Eurovent certified.
The composition of materials is the same for all sizes, and the ratio of materials is almost equal among the sizes. Key EPD data for the full range is
provided in the following table, including suggested conversion factors.
Size specific EPDs are also available upon request.
3 / 14
Size Weight [kg] GWPtot (A1-A3) [kg CO2 eq] Factor [-]
11 646,25 3897,92 0,564
12 732,23 4348,09 0,629
14 879,68 5105,87 0,738
16 1106,61 6330,53 0,916
18 1216,28 6914,01 1,000
20 1485,38 8290,85 1,199
22 1771,59 9853,78 1,425
24 2051,28 11275,27 1,631
27 2597,53 14475,16 2,094
29 2889,39 16147,84 2,336
31 3609,55 20517,40 2,968
10 584,65 3549,01 0,562
Market:
Europe
Reference service life, product
Determined by the application of the product.
Reference service life, building or construction works
Not declared.
LCA: Calculation rules
Declared unit:
1 pcs Geniox GO (R-HW-Optimized)
Cut-off criteria:
All major raw materials and all the essential energy is included. The production processes for raw materials and energy flows with very small
amounts (less than 1%) are not included. These cut-off criteria do not​ apply for hazardous materials and substances.
Allocation:
The allocation is made in accordance with the provisions of EN 15804. Energy, water and waste production in-house is allocated equally among all
products through mass allocation. Effects of primary production of recycled materials is allocated to the main product in which the material was
used. The recycling process and transportation of the material is allocated to this analysis.
Data quality:
Specific data for the product composition are provided by the manufacturer. The data represent the production of the declared product and were
collected for EPD development in the year of study. Background data is based on EPDs according to EN 15804 and different LCA databases. The
data quality of the raw materials in A1 is presented in the table below.
4 / 14
Materials Source Data quality Year
Adhesive ecoinvent 3.6 Database 2019
Chemical ecoinvent 3.6 Database 2019
Electronic - Unspecified ecoinvent 3.6 Database 2019
Filter, plastic based Modified ecoinvent 3.6 Database 2019
Glass fibre reinforced plastic, polyamide Modified ecoinvent 3.6 Database 2019
Hydronic coil (50% AL, 50%CU) ecoinvent 3.6 Database 2019
Insulation, Mineral based ecoinvent 3.6 Database 2019
Metal - Aluminium ecoinvent 3.6 Database 2019
Metal - Copper ecoinvent 3.6 Database 2019
Metal - Galvanized Steel ecoinvent 3.6 Database 2019
Metal - Steel ecoinvent 3.6 Database 2019
Metal - Steel Modified ecoinvent 3.6 Database 2019
Metal - Steel with aluzinc coating ecoinvent 3.6 Database 2019
Metal - Steel with magnelis coating ecoinvent 3.6 Database 2019
Motor ecoinvent 3.6 Database 2019
Motor Modified ecoinvent 3.6 Database 2019
Supplier data +
Other Material composition + ecoinvent 3.6 2019
database
Packaging - Paper ecoinvent 3.6 Database 2019
Packaging - Plastic ecoinvent 3.6 Database 2019
Plastic - Acrylonitrile butadiene styrene (ABS) ecoinvent 3.6 Database 2019
Plastic - Polyamide ecoinvent 3.6 Database 2019
Plastic - Polycarbonate (PC) ecoinvent 3.6 Database 2019
Plastic - Polyethylene ecoinvent 3.6 Database 2019
Plastic - Polyethylene (HDPE) ecoinvent 3.6 Database 2019
Plastic - Polypropylene (PP) ecoinvent 3.6 Database 2019
Plastic - Polyvinyl chloride (PVC) ecoinvent 3.6 Database 2019
Plastics ecoinvent 3.6 Database 2019
Rubber, synthetic ecoinvent 3.6 Database 2019
5 / 14
System boundaries (X=included, MND=module not declared, MNR=module not relevant)
Construction Beyond the system
Product stage Use stage End of life stage
installation stage boundaries
A1 A2 A3 A4 A5 B1 B2 B3 B4 B5 B6 B7 C1 C2 C3 C4 D
X X X X MND MND MND MND MND MND MND MND X X X X X
System boundary:
Additional technical information:
Complete project specific technical documentation is generated using our AHU calculation software, SystemairCAD. Please refer to the Systemair
website for more information.
waR slairetam tropsnarT gnirutcafunaM tropsnarT ylbmessA e​sU ecnanetniaM riapeR tnemecalpeR tnemhsibrufeR lanoitarepO ygrene esu lanoitarepO esu retaw -eD noitcurtsnoc noitilomed tropsnarT etsaW gnissecorp lasopsiD -yrevoceR-esueR laitnetop-gnilcyceR
6 / 14
LCA: Scenarios and additional technical information
The following information describe the scenarios in the different modules of the EPD.
For A4 a generic transportation distance (EURO6 truck) of 1000 km is declared. True transportation distance can be provided in project specific
EPD.
For C2 a generic transportation distance (EURO6 truck) of 50 km is declared. True transportation distance can be provided in project specific EPD.
Capacity utilisation Value
Transport from production place to user (A4) Distance (km) Fuel/Energy Consumption Unit
(incl. return) % (Liter/tonne)
Truck, 16-32 tonnes, EURO 6 (km) 36,7 % 1000 0,043 l/tkm 43,00
De-construction demolition (C1) Unit Value
Demolition of building per kg of ventilation
kg/DU 1186,000000000
product (kg)
Capacity utilisation Value
Transport to waste processing (C2) Distance (km) Fuel/Energy Consumption Unit
(incl. return) % (Liter/tonne)
Truck, 16-32 tonnes, EURO 6 (km) 36,7 % 50 0,043 l/tkm 2,15
Waste processing (C3) Unit Value
Materials to recycling (kg) kg 912,95
Waste treatment per kg Plastics, from incineration
kg 46,12
(kg)
Waste treatment per kg Hazardous waste,
kg 3,20
incineration (kg)
Waste treatment per kg Polypropylene (PP),
kg 0,55
incineration (kg)
Waste treatment per kg Electronics scrap, Control
kg 8,68
units, incineration (kg)
Waste treatment per kg Polyethylene (PE),
kg 0,35
incineration (kg)
Waste treatment per kg Rubber, municipal
kg 11,83
incineration with fly ash extraction (kg)
Waste treatment per kg wire plastic, municipal
kg 0,069
incineration - C3 - RoW
Waste treatment per kg Polyvinylchloride (PVC),
kg 25,025
incineration with fly ash extraction (kg)
Waste treatment per kg Bulk iron waste, excluding
kg 65,000000000
reinforcement, sorting plant (kg)
Waste treatment per kg plastic, industrial
electronics, municipal incineration with fly ash kg 8,79
extraction (kg)
Disposal (C4) Unit Value
Waste, aluminium, to landfill (kg) kg 12,79
Waste, plastic, mixture, to landfill (kg) kg 55,72
Landfilling of ashes from incineration of Plastics,
kg 1,084
process per kg ashes and residues (kg)
Landfilling of ashes from incineration per kg
kg 0,60
Hazardous waste, from incineration (kg)
Waste, scrap steel, to landfill (kg) kg 79,88
Landfilling of ashes from incineration of
Polypropylene (PP), process per kg ashes and kg 0,016
residues (kg)
Landfilling of ashes from incineration of
Electronics scrap, Control units, process of ashes kg 6,090
and residues (kg)
Landfilling of ashes from incineration of
Polyethylene (PE), process per kg ashes and kg 0,012
residues (kg)
Landfilling of ashes from incineration of Rubber,
kg 0,61
municipal incineration with fly ash extraction (kg)
Landfilling of ashes from incineration per kg wire
kg 0,010
plastic, from municipal incineration (kg)
Waste treatment per kg Copper slag, to landfill,
kg 2,65
residual material landfill (kg)
Landfilling of ashes from incineration of
Polyvinylchloride (PVC), process per kg ashes and kg 3,98
residues (kg)
Waste, mineral wool, to landfil (kg) kg 43,26
Landfilling of ashes from incineration per kg
plastic, industrial electronics, From municipal kg 0,59
incineration with fly ash extraction (kg)
7 / 14
Benefits and loads beyond the system
Unit Value
boundaries (D)
Substitution of primary aluminium with net scrap
kg 163,33
(kg)
Substitution of electricity, in Norway (MJ) MJ 58,000051
Substitution of thermal energy, district heating, in
MJ 877,48
Norway (MJ)
Substitution of primary steel with net scrap (kg) kg 684,63
Substitution of primary copper with net scrap (kg) kg 15,35
8 / 14
LCA: Results
The LCA results are presented below for the declared unit defined on page 2 of the EPD document.
Environmental impact
Indicator Unit A1-A3 A4 C1 C2 C3 C4 D
GWP-total kg CO2 -eq 6,91E+03 1,99E+02 1,56E+00 9,94E+00 2,41E+02 9,19E+00 -2,28E+03
GWP-fossil kg CO2 -eq 6,85E+03 1,99E+02 1,56E+00 9,93E+00 2,41E+02 9,18E+00 -2,25E+03
GWP-biogenic kg CO2 -eq 3,21E+01 8,22E-02 2,93E-04 4,11E-03 4,55E-02 3,35E-03 -7,26E+00
GWP-luluc kg CO2 -eq 3,51E+01 7,07E-02 1,23E-04 3,53E-03 8,08E-03 7,69E-04 -2,81E+01
ODP kg CFC11 -eq 5,53E-04 4,50E-05 3,38E-07 2,25E-06 3,34E-06 6,11E-07 -3,71E-01
AP mol H+ -eq 6,11E+01 5,71E-01 1,64E-02 2,85E-02 7,04E-02 1,65E-02 -1,98E+01
EP-FreshWater kg P -eq 4,50E-01 1,59E-03 5,69E-06 7,93E-05 4,14E-04 4,09E-05 -1,44E-01
EP-Marine kg N -eq 7,49E+00 1,13E-01 7,22E-03 5,65E-03 2,21E-02 1,22E-02 -2,28E+00
EP-Terrestial mol N -eq 1,50E+02 1,26E+00 7,92E-02 6,32E-02 2,30E-01 6,23E-02 -2,56E+01
POCP kg NMVOC -eq 2,89E+01 4,84E-01 2,18E-02 2,42E-02 6,00E-02 1,89E-02 -9,48E+00
ADP-minerals&metals1 kg Sb-eq 2,71E+00 5,49E-03 2,40E-06 2,74E-04 1,69E-04 1,83E-05 -4,53E-02
ADP-fossil1 MJ 8,89E+04 3,00E+03 2,15E+01 1,50E+02 1,27E+02 4,63E+01 -2,52E+04
WDP1 m3 9,84E+05 2,90E+03 4,57E+00 1,45E+02 1,68E+03 3,94E+02 -7,91E+05
GWP-total = Global Warming Potential total; GWP-fossil = Global Warming Potential fossil fuels; GWP-biogenic = Global Warming Potential biogenic; GWP-luluc =
Global Warming Potential land use and land use change; ODP = Depletion potential of the stratospheric ozone layer; AP = Acidification potential, Accumulated
Exceedance; EP-freshwater = Eutrophication potential, fraction of nutrients reaching freshwater end compartment: EP-marine = Eutrophication potential, fraction of
nutrients reaching marine end compartment; EP-terrestrial = Eutrophication potential, Accumulated Exceedance; POCP = Formation potential of tropospheric ozone;
ADP-minerals&metals = Abiotic depletion potential for non-fossil resources; ADP-fossil = Abiotic depletion for fossil resources potential; WDP = Water (user)
deprivation potential, deprivation-weighted water consumption
"Reading example: 9,0 E-03 = 9,0*10-3 = 0,009"
*INA Indicator Not Assessed
1. The results of this environmental impact indicator shall be used with care as the uncertainties on these results are high or as there is limited experienced with the
indicator
Remarks to environmental impacts
This air handling unit uses electric energy for fan drive and recovers thermal energy via the rotary heat exchanger. These factors are highly project
specific, and the environmental impact will vary depending on:
- Climate / outdoor conditions
- Air volume
- External pressure drop
- Supply temperature
- Extract temperature
- Operating hours
- Electricity origin
- Etc.
Energy use and heat recovery are key factors in determining the environmental impact of this product and must be calculated with project specific
values. This can be done using our AHU calculation software, SystemairCAD. Please refer to the Systemair website for more information.
9 / 14
Additional environmental impact indicators
Indicator Unit A1-A3 A4 C1 C2 C3 C4 D
PM Disease incidence 5,81E-04 1,22E-05 4,33E-07 6,08E-07 5,06E-07 2,75E-07 -1,79E-04
IRP2 kgBq U235 -eq 3,37E+02 1,31E+01 9,22E-02 6,56E-01 5,75E-01 2,23E-01 -7,84E+01
ETP-fw1 CTUe 3,16E+05 2,23E+03 1,18E+01 1,11E+02 3,71E+03 8,01E+03 -1,21E+05
HTP-c1 CTUh 3,06E-05 0,00E+00 0,00E+00 0,00E+00 2,60E-08 6,41E-08 -8,10E-06
HTP-nc1 CTUh 3,32E-04 2,43E-06 1,07E-08 1,22E-07 1,29E-06 4,30E-06 -3,30E-05
SQP1 dimensionless 2,42E+04 2,10E+03 2,73E+00 1,05E+02 4,30E+01 1,42E+02 -1,84E+03
PM = Particulate Matter emissions; IRP = Ionizing radiation – human health; ETP-fw = Eco toxicity – freshwater; HTP-c = Human toxicity – cancer effects; HTP-nc =
Human toxicity – non cancer effects; SQP = Potential Soil Quality Index (dimensionless)
"Reading example: 9,0 E-03 = 9,0*10-3 = 0,009"
*INA Indicator Not Assessed
1. The results of this environmental impact indicator shall be used with care as the uncertainties on these results are high or as there is limited experienced with the
indicator
2. This impact category deals mainly with the eventual impact of low dose ionizing radiation on human health of the nuclear fuel cycle. It does not consider effects due
to possible nuclear accidents, occupational exposure nor due to radioactive waste disposal in underground facilities. Potential ionizing radiation from the soil, from
radon and from some construction materials is also not measured by this indicator.
10 / 14
Resource use
Indicator Unit A1-A3 A4 C1 C2 C3 C4 D
PERE MJ 1,50E+04 4,30E+01 1,16E-01 2,15E+00 1,67E+01 2,39E+00 -7,77E+03
PERM MJ 8,05E+00 0,00E+00 0,00E+00 0,00E+00 0,00E+00 0,00E+00 0,00E+00
PERT MJ 1,50E+04 4,30E+01 1,16E-01 2,15E+00 1,67E+01 2,39E+00 -7,77E+03
PENRE MJ 8,40E+04 3,00E+03 2,15E+01 1,50E+02 1,27E+02 4,63E+01 -2,52E+04
PENRM MJ 5,02E+03 0,00E+00 0,00E+00 0,00E+00 0,00E+00 0,00E+00 0,00E+00
PENRT MJ 8,90E+04 3,00E+03 2,15E+01 1,50E+02 1,27E+02 4,63E+01 -2,52E+04
SM kg 1,14E+02 0,00E+00 1,06E-02 0,00E+00 -1,22E+00 -1,19E+00 1,44E+02
RSF MJ 2,33E+02 1,54E+00 2,86E-03 7,69E-02 3,41E-01 5,27E-02 2,54E+01
NRSF MJ 1,97E+03 5,50E+00 4,21E-02 2,75E-01 -4,53E-02 2,03E-01 7,77E+02
FW m3 1,03E+02 3,21E-01 1,11E-03 1,61E-02 1,72E+00 6,68E-02 -3,95E+01
PERE = Use of renewable primary energy excluding renewable primary energy resources used as raw materials; PERM = Use of renewable primary energy resources used
as raw materials; PERT = Total use of renewable primary energy resources; PENRE = Use of non renewable primary energy excluding non-renewable primary energy
resources used as raw materials; PENRM = Use of non renewable primary energy resources used as raw materials; PENRT = Total use of non renewable primary energy
resources; SM = Use of secondary materials; RSF = Use of renewable secondary fuels; NRSF = Use of non-renewable secondary fuels; FW = Net use of fresh water
"Reading example: 9,0 E-03 = 9,0*10-3 = 0,009"
*INA Indicator Not Assessed
11 / 14
End of life - Waste
Indicator Unit A1-A3 A4 C1 C2 C3 C4 D
HWD kg 3,80E+01 1,55E-01 6,34E-04 7,74E-03 3,44E-02 1,81E+00 1,78E+00
NHWD kg 2,35E+03 1,46E+02 2,55E-02 7,30E+00 7,16E+00 2,04E+02 -7,49E+02
RWD kg 3,11E-01 2,05E-02 1,49E-04 1,02E-03 7,66E-05 1,86E-04 -7,41E-02
HWD = Hazardous waste disposed; NHWD = Non-hazardous waste disposed; RWD = Radioactive waste disposed
"Reading example: 9,0 E-03 = 9,0*10-3 = 0,009"
*INA Indicator Not Assessed
End of life - Output flow
Indicator Unit A1-A3 A4 C1 C2 C3 C4 D
CRU kg 0,00E+00 0,00E+00 0,00E+00 0,00E+00 0,00E+00 0,00E+00 0,00E+00
MFR kg 5,37E+02 0,00E+00 1,04E-02 0,00E+00 9,13E+02 2,10E-02 1,21E+02
MER kg 3,29E+01 0,00E+00 3,22E-05 0,00E+00 4,56E+01 2,84E-04 -7,20E-02
EEE MJ 2,72E+01 0,00E+00 1,10E-04 0,00E+00 6,29E+01 3,14E-01 6,58E+00
EET MJ 4,12E+02 0,00E+00 1,67E-03 0,00E+00 9,51E+02 4,75E+00 9,96E+01
CRU = Components for re-use; MFR = Materials for recycling; MER = Materials for energy recovery; EEE = Exported energy electrical; EET = Exported energy thermal
"Reading example: 9,0 E-03 = 9,0*10-3 = 0,009"
*INA Indicator Not Assessed
Biogenic Carbon Content
Indicator Unit At the factory gate
Biogenic carbon content in product kg C 0,00E+00
Biogenic carbon content in accompanying packaging kg C 9,52E-02
Note: 1 kg biogenic carbon is equivalent to 44/12 kg CO2
12 / 14
Additional requirements
Greenhouse gas emissions from the use of electricity in the manufacturing phase
National production mix from import, low voltage (production of transmission lines, in addition to direct emissions and losses in grid) of applied
electricity for the manufacturing process (A3).
Electricity mix Source Amount Unit
Electricity, Lithuania (kWh) ecoinvent 3.6 373,46 g CO2-eq/kWh
Dangerous substances
The product contains no substances on the REACH Candidate list at or above 100 ppm, 0,01 % by weight.
Indoor environment
The air handling unit is an essential component for obtaining good thermal and atmospheric conditions. An optimally sized and well-functioning
AHU will have direct positive effects on human health, wellbeing, and productivity and is a crucial prerequisite for achieving a healthy indoor
environment.
Additional Environmental Information
Additional environmental impact indicators required in NPCR Part A for construction products
Indicator Unit A1-A3 A4 C1 C2 C3 C4 D
GWPIOBC kg CO2 -eq 6,96E+03 1,99E+02 1,56E+00 9,94E+00 2,41E+02 6,90E+00 -2,57E+03
GWP-IOBC: Global warming potential calculated according to the principle of instantaneous oxidation. In order to increase the transparency of biogenic carbon​
contribution to climate impact, the indicator GWP-IOBC is required as it declares climate impacts calculated according to the principle of instantaneous oxidation.​
GWP-IOBC is also referred to as GWP-GHG in context to Swedish public procurement legislation.
13 / 14
Bibliography
ISO 14025:2010 Environmental labels and declarations - Type III environmental declarations - Principles and procedures.
ISO 14044:2006 Environmental management - Life cycle assessment - Requirements and guidelines.
EN 15804:2012+A2:2019 Environmental product declaration - Core rules for the product category of construction products.
ISO 21930:2017 Sustainability in buildings and civil engineering works - Core rules for environmental product declarations of construction
products.
ecoinvent v3, Allocation, cut-off by classification, Swiss Centre of Life Cycle Inventories.
Iversen et al., (2021) eEPD v2021.09 Background information for EPD generator tool system verification, LCA.no Report number: 07.21
Graafland and Iversen (2022) EPD generator for NPCR 030 Ventilation components, Background information for EPD generator application and
LCA data, LCA.no report number: 12.22
NPCR Part A: Construction products and services. Ver. 2.0. April 2021, EPD-Norge.
NPCR 030 Part B for Ventilation components, Ver. 1.0, 18.05.2021, EPD Norway.
Program operator and publisher Phone: +47 977 22 020
The Norwegian EPD Foundation e-mail: post@epd-norge.no
Post Box 5250 Majorstuen, 0303 Oslo, Norway web: www.epd-norge.no
Owner of the declaration: Phone: +370 340 601 65
UAB Systemair e-mail: info@systemair.lt
Linu g. 101, 20174 Ukmerge, Lithuania web: www.systemair.com/lt
Author of the Life Cycle Assessment Phone: +47 916 50 916
LCA.no AS e-mail: post@lca.no
Dokka 6A, 1671 Kråkerøy, Norway web: www.lca.no
Developer of EPD generator Phone: +47 916 50 916
LCA.no AS e-mail: post@lca.no
Dokka 6A, 1671 Kråkerøy, Norway web: www.lca.no
ECO Platform web: www.eco-platform.org
ECO Portal web: ECO Portal
14 / 14
