ENVIRONMENTAL PRODUCT DECLARATION
as per ISO 14025 and EN 15804+A1
Owner of the Declaration ArcelorMittal
Programme holder Institut Bauen und Umwelt e.V. (IBU)
Publisher Institut Bauen und Umwelt e.V. (IBU)
Declaration number EPD-ARC-20220192-CBA1-EN
Issue date 07.12.2022
Valid to 06.12.2027
Welded steel pipes
ArcelorMittal
www.ibu-epd.com | https://epd-online.com
Umwelt Produktdeklaration Name des Herstellers – Name des Produkts
General Information
ArcelorMittal Welded steel pipes
Programme holder Owner of the declaration
IBU – Institut Bauen und Umwelt e.V. ArcelorMittal
Hegelplatz 1 Tubular Products Europe
10117 Berlin 24-26, boulevard d'Avranches
Germany L 1160 Luxembourg
Phone: 00 34 656 786 729
E-mail address: constructube@arcelormittal.com
Website: https://tubular.arcelormittal.com/
Declaration number Declared product / declared unit
EPD-ARC-20220192-CBA1-EN 1 metric tonne of steel pipes.
This declaration is based on the product Scope:
category rules: The declaration applies to 1 metric tonne of steel pipes
Steel pipes for pressure applications, 11.2017 produced by ArcelorMittal.
(PCR checked and approved by the SVR)
The life cycle assessment is based on data from the
Issue date production and finishing process occurring in the
following ArcelorMittal production plants:
07.12.2022
 Lexy (FR),
 Iasi (RO),
Valid to
 Krakow (PL) and
06.12.2027
 Karvina (CZ)
Production has been modelled using annual production
data from the period 2019. The weighting of production
volumes of the different production sites is based on
2019 data.
The owner of the declaration shall be liable for the
underlying information and evidence; the IBU shall not
be liable with respect to manufacturer information, life
cycle assessment data and evidences.
The EPD was created according to the specifications
of EN 15804+A1. In the following, the standard will be
simplified as EN 15804.
Verification
The standard EN 15804 serves as the core PCR
Independent verification of the declaration and data
according to ISO 14025:2011
Dipl. Ing. Hans Peters internally x externally
(chairman of Institut Bauen und Umwelt e.V.)
Dr. Alexander Röder Vito D'Incognito
(Managing Director Institut Bauen und Umwelt e.V.)) (Independent verifier)
Product
Product description/Product definition to each other: welded cold-forming or welded hot-
This EPD describes the welded steel pipes produced stretch reduction.
by ArcelorMittal.
For the placing on the market of the products covered
It covers the non-alloy steel tubes for the conveyance by the standards EN 10224:2002/A1:2005, Non-alloy
of water and other aqueous liquids, the non-alloy steel steel tubes and fittings for the conveyance of water
tubes suitable for welding and threading (also called and other aqueous liquids - Technical delivery
gas pipes) and the alloy and non-alloy steel pressure conditions and EN 10255:2004+A1:2007, Non-alloy
pipes. These pipes can also have more general- steel tubes suitable for welding and threading.
purpose applications where pressure is low.
Technical delivery conditions in the European
In some cases, the manufacturing route is very similar Union/European Free Trade Association (EU/EFTA)
2 Environmental Product Declaration ArcelorMittal – Welded Steel Pipes
(with the exception of Switzerland) Regulation (EU) design needs.
No. 305/2011 (CPR) applies. These products need a
declaration of performance and the CE-marking. For a given product, the geometrical tolerances will be
fully controlled by the product standards (EN 10224,
For the application and use the respective national EN 10255 or EN 10217) and they will be consistent
provisions apply. with execution and design rules in order to assure a
safe and suitable system.
Other European standards concerning steel pipes
could also be used by manufacturers as reference:
Constructional data
 EN 10217-1:2019, Welded steel tubes for Name Value Unit
pressure purposes - Technical delivery Yield strength at room temperature 195 - N/mm2
460
conditions - Part 1: Electric welded and
320 -
submerged arc welded non-alloy steel tubes Tensile strength at room temperature N/mm2
730
with specified room temperature properties
Elongation at room temperature 17 - 25 %
 EN 10217-2:2019, Welded steel tubes for Minimum average absorbed energy at
27 - 35 Joule
pressure purposes - Technical delivery 0°C
conditions - Part 2: Electric welded non-alloy
and alloy steel tubes with specified elevated
temperature properties
 EN 10217-3:2019, Welded steel tubes for
Base materials/Ancillary materials
pressure purposes - Technical delivery
The basic materials for the manufacture of
conditions - Part 3: Electric welded and ArcelorMittal’s steel pipes are non-alloyed and fine-
submerged arc welded alloy fine grain steel grain steel. Different steel grades and qualities are
tubes with specified room, elevated and low- possible, these being recorded in the specific product
temperature properties. standards – EN 10224 or EN 10255.
Alloyed and non-alloyed steels can be found in pipes
Some of the aforementioned standards/products for pressure purposes – EN 10217. Different steel
comply with the Directive (EU) No. 2014/68 (PED) for grades and qualities are possible.
which CE-marking is not required.
Alloying elements are added in the form of ferroalloys
Application or metals (most common elements are Manganese
Welded steel pipes can be used in applications such and Silicon). Some small quantities of other elements
as transportation conveyance of water and gas, may be present in the steel.
transportation of pressured gases, and others.
Reference service life
Technical Data A reference service life for steel pipes is not declared.
The dimensions (wall thickness and outside These are construction or pressure products with many
dimensions), section properties (minimum yield different applications purposes. The lifetime therefore
strength, tensile strength, minimum elongation, will be limited by the service life of the work.
minimum impact energy) and chemical composition
vary according to the grade and quality of the steel to
be chosen and are also dependent on the piping
LCA: Calculation rules
Declared Unit
The declaration refers to the functional unit of 1 metric
ton of welded steel pipes as specified in Part B System boundary
requirements on the EPD for steel pipes for pressure Type of the EPD: cradle-to-gate - with options. Module
applications. A1-A3, module C3-C4 and module D were considered.
Foreground data for the production are integrated into Modules A1-A3 include the following:
the software model for the considered production  The provision of resources, additives, and
site/company. The LCI is assessed as per the annual energy
production data of ArcelorMittal Tubular Products
 Transport of resources and additives to the
Europe at the sites Iasi (Romania), Krakow (Poland),
production site
Karvina (Czechia) and Lexy (France). The background
data are taken from GaBi Documentation.  Production processes on site including
energy, production of additives, disposal of
production residues, and consideration of
related emissions.
Declared unit
 Recycling of production/manufacturing scrap.
Name Value Unit
Steel scrap is assumed to reach the end-of-
Declared unit 1 t
Density 7850 kg/m3 waste status once it is shredded and sorted,
3 Environmental Product Declaration ArcelorMittal – Welded Steel Pipes
thus becoming input to the product system in Comparability
the inventory. Basically, a comparison or an evaluation of EPD data
is only possible if all the data sets to be compared
were created according to EN 15804 and the building
Module C3-C4 take into account the sorting and
context, respectively the product-specific
shredding of after-use steel, as well as the non-
characteristics of performance, are taken into account.
recovered scrap due to sorting efficiency which is
landfilled. A conservative value of 10% landfill is
considered.
For the life cycle modelling of the product under study,
the GaBi Software System for Life Cycle Engineering,
Module D refers to the End-of-Life, including recycling.
content version 2021.2, is used (GaBi).
LCA: Scenarios and additional technical information
Current practice for the average pipe product consists
of 93 % recycling and 7 % reuse according to
SteelConstruction-info.
This EPD considers 90 % recycling and 10 % landfill
as a conservative approach.
End of life (C1-C4)
Name Value Unit
Landfilling 10 %
Reuse, recovery and/or recycling potentials (D),
relevant scenario information
Name Value Unit
Recycling 90 %
4 Environmental Product Declaration ArcelorMittal – Welded Steel Pipes
LCA: Results
DESCRIPTION OF THE SYSTEM BOUNDARY (X = INCLUDED IN LCA; MND = MODULE NOT DECLARED;
MNR = MODULE NOT RELEVANT)
BENEFITS AND
CONSTRUCTI LOADS
PRODUCT STAGE ON PROCESS USE STAGE END OF LIFE STAGE BEYOND THE
STAGE SYSTEM
BOUNDARIES
5 Environmental Product Declaration ArcelorMittal – Welded Steel Pipes
lairetam
waR
ylppus tropsnarT
gnirutcafunaM
eht
morf
tropsnarT
etis
eht
ot
etag
ylbmessA esU
ecnanetniaM
riapeR
tnemecalpeR tnemhsibrufeR
ygrene
lanoitarepO esu
retaw
lanoitarepO esu
noitcurtsnoc-eD
noitilomed tropsnarT
gnissecorp
etsaW
lasopsiD -esueR -yrevoceR -gnilcyceR laitnetop
A1 A2 A3 A4 A5 B1 B2 B3 B4 B5 B6 B7 C1 C2 C3 C4 D
X X X MND MND MND MND MNR MNR MNR MND MND MND MND X X X
RESULTS OF THE LCA - ENVIRONMENTAL IMPACT according to EN 15804+A1: 1 ton Welded Steel Pipes
Parameter Unit A1-A3 C3 C4 D
Global warming potential [kg CO2-Eq.] 2.80E+3 1.60E+0 1.43E+0 -1.32E+3
Depletion potential of the stratospheric ozone layer [kg CFC11-Eq.] 3.65E-12 4.69E-14 7.83E-15 -4.39E-12
Acidification potential of land and water [kg SO2-Eq.] 5.14E+0 2.99E-3 8.57E-3 -2.05E+0
Eutrophication potential [kg (PO4)3--Eq.] 4.82E-1 4.48E-4 9.72E-4 -1.49E-1
Formation potential of tropospheric ozone photochemical
[kg ethene-Eq.] 8.72E-1 2.60E-4 6.58E-4 -6.12E-1
oxidants
Abiotic depletion potential for non-fossil resources [kg Sb-Eq.] 5.44E-2 4.70E-7 1.44E-7 -3.43E-3
Abiotic depletion potential for fossil resources [MJ] 2.75E+4 1.82E+1 1.95E+1 -1.37E+4
RESULTS OF THE LCA - INDICATORS TO DESCRIBE RESOURCE USE according to EN 15804+A1: 1 ton
Welded Steel Pipes
Parameter Unit A1-A3 C3 C4 D
Renewable primary energy as energy carrier [MJ] 1.30E+3 1.22E+1 2.70E+0 8.52E+2
Renewable primary energy resources as material utilization [MJ] 0.00E+0 0.00E+0 0.00E+0 0.00E+0
Total use of renewable primary energy resources [MJ] 1.30E+3 1.22E+1 2.70E+0 8.52E+2
Non-renewable primary energy as energy carrier [MJ] 2.87E+4 2.82E+1 2.01E+1 -1.35E+4
Non-renewable primary energy as material utilization [MJ] 0.00E+0 0.00E+0 0.00E+0 0.00E+0
Total use of non-renewable primary energy resources [MJ] 2.87E+4 2.82E+1 2.01E+1 -1.35E+4
Use of secondary material [kg] 8.53E+1 0.00E+0 0.00E+0 0.00E+0
Use of renewable secondary fuels [MJ] 0.00E+0 0.00E+0 0.00E+0 0.00E+0
Use of non-renewable secondary fuels [MJ] 0.00E+0 0.00E+0 0.00E+0 0.00E+0
Use of net fresh water [m³] 1.33E+1 1.18E-2 4.95E-3 -8.80E+1
RESULTS OF THE LCA – WASTE CATEGORIES AND OUTPUT FLOWS according to EN 15804+A1:
1 ton Welded Steel Pipes
Parameter Unit A1-A3 C3 C4 D
Hazardous waste disposed [kg] 1.10E-5 6.99E-9 2.13E-9 2.96E-6
Non-hazardous waste disposed [kg] 5.65E+1 1.89E-2 1.00E+2 1.73E+2
Radioactive waste disposed [kg] 3.56E-1 3.89E-3 2.10E-4 1.47E-3
Components for re-use [kg] 0.00E+0 0.00E+0 0.00E+0 0.00E+0
Materials for recycling [kg] 0.00E+0 9.00E+2 0.00E+0 0.00E+0
Materials for energy recovery [kg] 0.00E+0 0.00E+0 0.00E+0 0.00E+0
Exported electrical energy [MJ] 0.00E+0 0.00E+0 0.00E+0 0.00E+0
Exported thermal energy [MJ] 0.00E+0 0.00E+0 0.00E+0 0.00E+0
References
Standards: alloy steel tubes with specified room temperature
properties
Directive (EU) No. 2014/68 (PED)
Directive 2014/68/EU of the European Parliament and EN 10216-2
of the Council of 15 May 2014 on the harmonisation of EN 10216-2:2013+A1:2019, Seamless steel tubes for
the laws of the Member States relating to the making pressure purposes - Technical delivery conditions -
available on the market of pressure equipment (recast) Part 2: Non-alloy and alloy steel tubes with specified
Text with EEA relevance. elevated temperature properties
EN 10216-1 EN 10216-3
EN 10216-1:2013, Seamless steel tubes for pressure EN 10216-3:2013, Seamless steel tubes for pressure
purposes - Technical delivery conditions - Part 1: Non- purposes - Technical delivery conditions - Part 3: Alloy
fine grain steel tubes
DIN EN ISO 14025:2011-10, Environmental labels and
EN 10216-4 declarations — Type III environmental declarations —
EN 10216-4:2013, Seamless steel tubes for pressure Principles and procedures.
purposes - Technical delivery conditions - Part 4: Non-
alloy and alloy steel tubes with specified low Regulation (EU) No. 305/2011 (CPR)
temperature properties Regulation (EU) no 305/2011 of the European
parliament and of the council of 9 March 2011.
EN 10217-1 Laying down harmonized conditions for the marketing
EN 10217-1:2019, Welded steel tubes for pressure of construction products and repealing council directive
purposes - Technical delivery conditions - Part 1: 89/106/EEC.
Electric welded and submerged arc welded non-alloy
steel tubes with specified room temperature properties Other References:
EN 10217-2 GaBi
EN 10217-2:2019, Welded steel tubes for pressure GaBi dataset documentation for the GaBi Software
purposes - Technical delivery conditions - Part 2: System and Database for Life Cycle Engineering,
Electric welded non-alloy and alloy steel tubes with thinkstep AG, Leinfelden-Echterdingen, 2021
specified elevated temperature properties (http://documentation.gabi-software.com/)
EN 10217-3 IBU 2021
EN 10217-3:2019, Welded steel tubes for pressure General Instructions for the EPD programme of Institut
purposes - Technical delivery conditions - Part 3: Bauen und Umwelt e.V. Version 2.0, Berlin: Institut
Electric welded and submerged arc welded alloy fine Bauen und Umwelt e.V., 2021. www.ibuepd.com
grain steel tubes with specified room, elevated and low
temperature properties PCR Part A
PCR - Part A: Calculation rules for the Life Cycle
EN 10224/A1 Assessment and Requirements on the Background
EN 10224:2002/A1:2005, Non-alloy steel tubes and Report, version 1.8, Institut Bauen und Umwelt e.V.,
fittings for the conveyance of water and other aqueous www.bau-umwelt.com, 2019
liquids - Technical delivery conditions
PCR Part B
EN 10255+A1 PCR – Part B: Requirements of the EPD for Steel
EN 10255:2004+A1:2007, Non-alloy steel tubes Pipes for Pressure Applications, Institut Bauen und
suitable for welding and threading. Technical delivery Umwelt e.V., www.bau-umwelt.com, 2017
conditions
SteelConstruction-info
EN 15804 https://www.steelconstruction.info/The_recycling_and_
EN 15804:2012-04+A1 2013, Sustainability of reuse_survey
construction works — Environmental Product
Declarations — Core rules for the product category of
construction products.
ISO 14025
6 Environmental Product Declaration ArcelorMittal – Welded Steel Pipes
Publisher
Institut Bauen und Umwelt e.V. Tel +49 (0)30 3087748- 0
Hegelplatz 1 Fax +49 (0)30 3087748- 29
10117 Berlin Mail info@ibu-epd.com
Germany Web www.ibu-epd.com
Programme holder
Institut Bauen und Umwelt e.V. Tel +49 (0)30 - 3087748- 0
Hegelplatz 1 Fax +49 (0)30 – 3087748 - 29
10117 Berlin Mail info@ibu-epd.com
Germany Web www.ibu-epd.com
Author of the Life Cycle
Assessment Tel Nummer
Name Fax Nummer
Straße, Nr. Mail e-mail
PLZ, Ort Web Web-Adresse
Land
Owner of the Declaration
ArcelorMittal Europe Tubular Tel 00 34 656 786 729
Products Europe Fax -
boulevard d'Avranches 24-26 Mail constructube@arcelormittal.com
1160 Luxembourg Web
Luxembourg https://tubular.arcelormittal.co
m/
