ENVIRONMENTAL PRODUCT DECLARATION
as per ISO 14025 and EN 15804+A2
Owner of the Declaration Gemeinschaft umweltfreundlicher Teppichboden (GUT) e.V.
Programme holder Institut Bauen und Umwelt e.V. (IBU)
Publisher Institut Bauen und Umwelt e.V. (IBU)
Declaration number EPD-GUT-20220345-CBG1-EN
Issue date 01.02.2023
Valid to 31.01.2028
Tufted wall-to-wall carpet - luxury class LC1
with a pile material made of polyamide 6 with 100%
recycled content
maximum surface pile weight 400 g/m2,
maximum total pile weight 650 g/m2,
textile backing with a maximum weight of 250 g/m2
Gemeinschaft umweltfreundlicher
Teppichboden (GUT)
www.ibu-epd.com | https://epd-online.com
Umwelt Produktdeklaration Name des Herstellers – Name des Produkts
General Information
Gemeinschaft umweltfreundlicher Tufted wall-to-wall carpet - luxury
Teppichboden (GUT) e.V. class LC1, with PA 6 pile material
with 100% recycled content, max.
surface pile weight 400 g/m2, max.
total pile weight 650 g/m2, textile
backing with a max. weight of 250 g/m2
Programme holder Owner of the declaration
IBU – Institut Bauen und Umwelt e.V. Gemeinschaft umweltfreundlicher Teppichboden e.V.
Hegelplatz 1 Schönebergstraße 2
10117 Berlin 51068 Aachen
Germany Germany
Declaration number Declared product / declared unit
EPD-GUT-20220345-CBG1-EN 1 m² tufted wall-to-wall carpet, luxury class LC1, PA 6
pile material with 100% recycled content, textile
backing.
This declaration is based on the product Scope:
category rules: This sample EPD applies to all products of the member
Floor coverings, 02/2018 companies of the Gemeinschaft umweltfreundlicher
(PCR checked and approved by the SVR) Teppichboden (GUT) e.V. that comply with the product
descriptions and are registered in the GUT/PRODIS
information system. It is only valid in conjunction with a
Issue date
valid GUT/PRODIS license of the product.
01.02.2023
The construction and production data of the registered
products are provided by the member companies of
Valid to
the GUT e.V.. The production sites are located in
31.01.2028 Belgium, Denmark, France, Germany, the Netherlands
and Switzerland.
The owner of the declaration shall be liable for the
underlying information and evidence; the IBU shall not
be liable with respect to manufacturer information, life
cycle assessment data and evidences.
The EPD was created according to the specifications
of EN 15804+A2. In the following, the standard will be
simplified as EN 15804.
Verification
The standard EN 15804 serves as the core PCR
Independent verification of the declaration and data
according to ISO 14025:2011
Dipl. Ing. Hans Peters internally x externally
(chairman of Institut Bauen und Umwelt e.V.)
Dr. Alexander Röder Angela Schindler
(Managing Director Institut Bauen und Umwelt e.V.)) (Independent verifier)
Product
Product description/Product definition Colouring and design of the use layer may be achieved
The declaration applies to tufted wall-to-wall carpets by aqueous dyeing methods or by using solution-dyed
having a pile material of polyamide 6 with 100% yarns.
recycled content and a textile backing with a maximum For the placing on the market of the specific product in
weight of 250 g/m2. the European Union/European Free Trade Association
The total recycled content of the carpet is 27%. (EU/EFTA) (with the exception of Switzerland)
The products correspond to luxury class LC1 with a Regulation (EU) No. 305/2011 Construction Product
limitation of the maximum surface pile weight of 400 Regulation (CPR) applies. The product needs a
g/m² and a maximum total pile weight of 650 g/m2. Declaration of Performance (DoP) taking into
consideration EN 14041:2018-05, Resilient, textile and
laminate floor coverings - Essential characteristics, and
2 Environmental Product Declaration GUT e.V. – Tufted wall-to-wall carpet with 100% recycled PA6 pile material and textile
backing, LC1
the CE-marking. The DoP of the product can be found Polypropylene 7.9 %
on the manufacturer's technical information section. Mineral Filler 38.9 %
For the application and use of the product the Aluminiumhydroxide 6.3 %
respective national provisions apply. Polymer dispersion (solid content) 7.6 %
Additives 4.3 %
Application The base materials refer to the fictitious worst-case
The use class of the specific product as defined in product representing all products with the described
EN 1307 can be found in the Product Information characteristics.
System (PRODIS) using the PRODIS registration The specific product covered by the EPD contains
number of the product. substances listed in the ECHA candidate list
(08.07.2021) or other carcinogenic, mutagenic or
Technical Data
reprotoxic (CMR) substances in categories 1A or 1B
The technical data describes a fictitious worst-case which are not on the candidate list exceeding 0.1
product representing all products with the described percentage by mass: no
characteristics. The products are registered in the GUT-PRODIS
Information System. The PRODIS system ensures the
Constructional data according to EN 1307 compliance with limitations of various chemicals and
Name Value Unit Volatile Organic Compound (VOC)-emissions and a
Product Form wall-to-wall carpet on rolls -
ban on the use of all substances that are listed as
Type of Tufted carpet - 'Substances of Very High Concern' (SVHC) under
manufacture REACH.
Polyamide 6 with 100%
Yarn type -
recycled content Reference service life
Total carpet weight max. 2400 g/m2 The service life of textile floor coverings strongly
Surface pile weight max. 400 g/m2 depends on the correct installation taking into account
Secondary backing Textile backing - the declared use classification and the adherence to
cleaning and maintenance instructions.
A calculation of the reference service life according to
Performance data of the product in accordance with ISO 15686 is not possible.
the declaration of performance with respect to its Alternatively, a reference service life of 10 years can
essential characteristics according to EN 14041: 2018- be assumed, during which the functional and visual
05, Resilient, textile and laminate floor coverings - quality is guaranteed (BNB, Nutzungsdauer von
Essential characteristics. Bauteilen). The technical service life can be
Additional product properties in accordance with EN significantly longer.
1307 can be found on the Product Information System
PRODIS using the PRODIS registration number of the
product (www.pro-dis.info) or on the manufacturer's
technical information section.
Base materials/Ancillary materials
Name Value Unit
Polyamide 6 27.1 %
Polyester 7.9 %
LCA: Calculation rules
Declared Unit System boundary
Type of EPD:
Name Value Unit Cradle-to-gate with options, module C1-C4, module D,
Declared unit 1 m2 and additional modules A4, A5, B1, B2.
Grammage 2.4 kg/m2
The declared unit refers to 1 m2 produced textile floor System boundaries of modules A, B, C, D:
covering. The Output of module A5 'Assembly' is 1 m2 Modules C3, C4 and D are indicated separately for
installed textile floor covering. three end-of-life scenarios:
The layer thickness of the specific product covered by 1 - landfill disposal
the EPD can be found on the Product Information 2 - municipal waste incineration
System PRODIS using the PRODIS registration 3 - recovery in a cement plant
number of the product (www.pro-dis.info) or on the
manufacturer's technical information section. A1-A3 Production:
Energy supply and production of the basic material,
The LCA results refer to the fictitious worst-case processing of secondary material, auxiliary material,
product, which covers all products of the members of transport of the material to the manufacturing site,
the GUT e.V. that correspond to the product emissions, waste water treatment, packaging material
descriptions and are registered in the GUT/PRODIS and waste processing up to the landfill disposal of
information system. residual waste (except radioactive waste). Benefits for
generated electricity and steam due to the incineration
of production waste are aggregated.
Biogenic carbon that is stored in renewable material
3 Environmental Product Declaration GUT e.V. – Tufted wall-to-wall carpet with 100% recycled PA6 pile material and textile
backing, LC1
(packaging paper) is taken into account as well as the
associated carbon dioxide uptake from the air from C1 De-construction:
which this biogenic carbon comes. The floor covering is de-constructed manually and no
additional environmental impact is caused.
A4 Transport:
Transport of the packed textile floor covering C2 Transport:
from factory gate to the place of installation. Transport of the carpet waste to a landfill, to the
municipal waste incineration plant (MWI) or to the
waste collection facility for recycling.
C3 Waste processing:
A5 Installation: C3-1: Landfill disposal needs no waste processing.
Installation of the textile floor covering, processing of C3-2: Impact from waste incineration (plant with
installation waste and packaging waste up to the R1>0.6), generated electricity and steam are listed in
landfill disposal of residual waste (except radioactive the result table as exported energy.
waste), the production of the amount of carpet that C3-3: Collection of the carpet waste for recovery in the
occurs as installation waste including its transport to cement industry, waste processing (granulating),
the place of installation. transport to the cement plant, emissions from the
Generated electricity and steam due to the incineration incineration.
of waste are listed in the result table as exported
energy. C4 Disposal
Biogenic carbon that is stored in renewable materials C4-1: Impact from landfill disposal,
in packaging paper is released as carbon dioxide C4-2: The carpet waste leaves the system in
emissions into the air at the end of life in module A5. module C3-2,
Preparation of the floor and auxiliary materials C4-3: The pre-processed carpet waste leaves the
(adhesives, fixing agents, PET connectors) are beyond system in module C3-3.
the system boundaries and not taken into account.
D Recycling potential:
B1 Use: Calculated benefits result from materials exclusive
Indoor emissions during the use stage. After the first secondary materials (net materials).
year, no product-related Volatile Organic Compound D-A5: Benefits for generated energy due
(VOC) emissions are relevant due to known VOC to incineration of packaging and installation waste
decay curves of the product. (incineration plant with R1 > 0.6),
D-1: Benefits for generated energy due to landfill
B2 Maintenance: disposal of carpet waste at the end of life,
Cleaning of the textile floor covering for a period of 1 D-2: Benefits for generated energy due to incineration
year: of carpet waste at the end-of-life (incineration plant
Vacuum cleaning – electricity supply with R1 > 0.6),
Wet cleaning – electricity, water consumption, D-3: Benefits for saved fossil energy and saved
production of the cleaning agent, waste water inorganic material due to recovery of the carpet in a
treatment. cement plant.
The declared values in this module have to be
multiplied by the assumed service life of the floor Comparability
covering in the building in question. Basically, a comparison or an evaluation of EPD data
is only possible if all the data sets to be compared
B3 - B5: were created according to EN 15804 and the building
The modules are not relevant within the assumed context, respectively the product-specific
reference service life of 10 years. characteristics of performance, are taken into account.
B6 - B7: Background data are taken from the GaBi database,
No energy and water input are required for the 2021-2. Remaining data gaps are covered by the
operation of the carpet in the use stage. The modules ecoinvent 3.7 database, 2020.
are not relevant and not declared.
LCA: Scenarios and additional technical information
Characteristic product properties Litres of fuel (truck, EURO 0-6
0.0057 l/100km
Information on biogenic carbon mix)
Transport distance 700 km
Capacity utilisation (including
55 %
Name Value Unit empty runs)
Biogenic carbon content in
accompanying packaging at factory 0.005 kg C Installation in the building (A5)
gate Name Value Unit
1 kg biogenic Carbon is equivalent to 44/12 kg of CO 2 Material loss 0.216 kg
Polyethylene packaging waste and installation waste
are considered to be incinerated in a municipal waste
incineration plant. Cardboard packaging waste is going
Transport to the construction site (A4) to be recycled.
Name Value Unit Preparation of the floor and auxiliaries (adhesives,
4 Environmental Product Declaration GUT e.V. – Tufted wall-to-wall carpet with 100% recycled PA6 pile material and textile
backing, LC1
fixing agents, PET connectors etc.) are not taken into + z % impact (Scenario 3)
account. with x % + y % + z % = 100 %
Maintenance (B2) Name Value Unit
The values for cleaning refer to 1 m2 floor covering per Collected as mixed construction
2.4 kg
year. waste (scenarios 1 and 2)
Depending on the application based on ISO 10874, the Collected separately (scenario 3) 2.4 kg
technical service life recommended by the Landfilling (scenario 1) 2.4 kg
manufacturer and the anticipated strain on the floor by Energy recovery (scenario 2) 2.4 kg
customers, the case-specific useful life can be Energy recovery (scenario 3) 1.316 kg
established. Based on this useful life the effects of Recycling (scenario 3) 1.084 kg
module B2 need to be calculated in order to obtain the
overall environmental impacts. Reuse, recovery and/or recycling potentials (D),
relevant scenario information
Recovery or recycling potentials due to the three end
Name Value Unit of life scenarios (module C) are indicated separately.
Maintenance cycle (vacuum Number
156
cleaning) /year
Recycling in the cement industry (scenario 3)
Maintenance cycle (wet cleaning) 0.92 Number The organic material of the carpet is used as an
/year alternative fuel in a cement kiln. It mainly substitutes
Water consumption (wet cleaning) 0.0027 m3 for lignite (68.8 %), hard coal (23.6 %) and petrol coke
Cleaning agent (wet cleaning) 0.055 kg (7.6 %). The inorganic material is substantially
Electricity consumption 0.326 kWh integrated into the cement clinker and substitutes for
The values result from the calculation of a mixed the original material input. VDZ e.V.
scenario for use in object areas and in private areas.
Maintenance cycle vacuum cleaning: 4 times per week
in object areas, 2 times per week in private areas.
Maintenance cycle wet cleaning: 3 times per 2 years in
object areas, 1 time per 3 years in private areas.
Service life
Name Value Unit
Life Span (according to BBSR) 10 a
Correspon
ds to the
Declared product properties (at
specificatio -
the gate) and finishes
ns of EN
1307
Conforms
An assumed quality of work, when to the
installed in accordance with the manufactur -
manufacturer’s instructions er's
instructions
Use in
areas
defined by
Usage conditions, e.g. frequency
the use -
of use, mechanical exposure
class
according
to EN 1307
According
Maintenance e.g. required to the
frequency, type and quality and manufactur -
replacement of components ers'
instructions
End of Life (C1-C4)
Three different end-of-life scenarios are declared and
the results are indicated separately in module C.
Each scenario is calculated as a 100 % scenario.
Scenario 1: 100 % landfill disposal
Scenario 2: 100 % municipal waste incineration (MWI)
with R1>0.6
Scenario 3: 100 % recovery in the cement industry
If combinations of these scenarios have to be
calculated this should be done according to the
following scheme:
EOL-impact = x % impact (Scenario 1)
+ y % impact (Scenario 2)
5 Environmental Product Declaration GUT e.V. – Tufted wall-to-wall carpet with 100% recycled PA6 pile material and textile
backing, LC1
LCA: Results
The modules C3/1, C4/2 and C4/3 cause no additional impact (see chapter "LCA: Calculation rules").
Module C2 represents the transport for scenarios 1, 2 and 3. The values in column D result from module A5.
DESCRIPTION OF THE SYSTEM BOUNDARY (X = INCLUDED IN LCA; ND = MODULE OR INDICATOR NOT
DECLARED; MNR = MODULE NOT RELEVANT)
BENEFITS AND
CONSTRUCTI LOADS
PRODUCT STAGE ON PROCESS USE STAGE END OF LIFE STAGE BEYOND THE
STAGE SYSTEM
BOUNDARIES
6 Environmental Product Declaration GUT e.V. – Tufted wall-to-wall carpet with 100% recycled PA6 pile material and textile
backing, LC1
lairetam
waR
ylppus tropsnarT
gnirutcafunaM
eht
morf
tropsnarT
etis
eht
ot
etag
ylbmessA esU
ecnanetniaM
riapeR
tnemecalpeR tnemhsibrufeR
ygrene
lanoitarepO esu
retaw
lanoitarepO esu
noitcurtsnoc-eD
noitilomed tropsnarT
gnissecorp
etsaW
lasopsiD -esueR -yrevoceR -gnilcyceR laitnetop
A1 A2 A3 A4 A5 B1 B2 B3 B4 B5 B6 B7 C1 C2 C3 C4 D
X X X X X X X MNR MNR MNR ND ND X X X X X
RESULTS OF THE LCA - ENVIRONMENTAL IMPACT according to EN 15804+A2: 1 m² floor covering
Core Indicator Unit A1-A3 A4 A5 B1 B2 C1 C2 C3/2 C3/3 C4/1 D D/1 D/2 D/3
GWP-total [kg CO2-Eq.] 5.29E+01.48E-11.05E+00.00E+03.85E-10.00E+08.14E-33.48E+03.52E+01.70E-1-1.59E-10.00E+0-5.45E-1-1.53E-1
GWP-fossil [kg CO2-Eq.] 5.28E+01.45E-11.04E+00.00E+02.62E-10.00E+07.99E-33.48E+03.52E+01.70E-1-1.58E-10.00E+0-5.43E-1-1.53E-1
GWP-biogenic [kg CO2-Eq.] 8.80E-3 1.88E-3 8.94E-30.00E+02.99E-30.00E+01.03E-4 3.96E-4 7.66E-4 2.04E-8-8.07E-40.00E+0-2.73E-3-1.30E-4
GWP-luluc [kg CO2-Eq.] 4.57E-3 8.20E-4 4.99E-40.00E+01.20E-10.00E+04.54E-5 1.13E-4 2.29E-4 8.28E-5-1.74E-50.00E+0-5.85E-5-8.12E-5
8.83E- 7.04E- 4.87E- 2.55E- 4.36E- 2.29E- -1.07E- -3.57E- -2.23E-
ODP [kg CFC11-Eq.] 7.82E-9 0.00E+02.08E-80.00E+0 0.00E+0
15 10 16 13 13 13 12 12 13
AP [mol H+-Eq.] 1.36E-2 8.78E-4 1.60E-30.00E+06.17E-40.00E+04.82E-5 3.09E-3 3.24E-3 5.04E-4-2.07E-40.00E+0-7.04E-4-5.90E-4
EP-freshwater [kg P-Eq.] 4.30E-5 4.40E-7 3.95E-60.00E+03.31E-60.00E+02.42E-8 4.09E-7 5.05E-7 3.17E-5-2.17E-70.00E+0-7.30E-7-1.94E-7
EP-marine [kg N-Eq.] 4.49E-3 4.30E-4 5.86E-40.00E+01.45E-40.00E+02.37E-5 1.52E-3 1.58E-3 1.12E-4-5.64E-50.00E+0-1.92E-4-1.80E-4
EP-terrestrial [mol N-Eq.] 4.26E-2 4.77E-3 5.92E-30.00E+01.98E-30.00E+02.64E-4 1.71E-2 1.78E-2 1.22E-3-6.03E-40.00E+0-2.06E-3-1.97E-3
POCP [kg NMVOC-Eq.]1.22E-2 8.13E-4 1.54E-3 4.18E-4 6.66E-40.00E+04.49E-5 3.89E-3 4.02E-3 3.58E-4-1.57E-40.00E+0-5.39E-4-5.33E-4
6.79E-
ADPE [kg Sb-Eq.] 1.41E-6 1.23E-8 1.30E-70.00E+01.54E-70.00E+0 1.41E-8 1.92E-8 1.18E-8-2.38E-80.00E+0-8.06E-8-1.55E-8
10
- - -
ADPF [MJ] 1.04E+21.97E+09.73E+00.00E+04.50E+00.00E+01.09E-11.70E+02.19E+02.42E+0 0.00E+0
2.69E+0 9.21E+01.72E+1
[m³ world-Eq
WDP 4.13E+01.32E-3 4.32E-10.00E+07.22E-20.00E+07.27E-5 4.31E-1 4.34E-1-1.81E-3-1.66E-20.00E+0-5.59E-2-2.17E-2
deprived]
GWP = Global warming potential; ODP = Depletion potential of the stratospheric ozone layer; AP = Acidification potential of land and water; EP =
Caption Eutrophication potential; POCP = Formation potential of tropospheric ozone photochemical oxidants; ADPE = Abiotic depletion potential for non-
fossil resources; ADPF = Abiotic depletion potential for fossil resources; WDP = Water (user) deprivation potential
RESULTS OF THE LCA - INDICATORS TO DESCRIBE RESOURCE USE according to EN 15804+A2: 1 m²
floor covering
Indicator Unit A1-A3 A4 A5 B1 B2 C1 C2 C3/2 C3/3 C4/1 D D/1 D/2 D/3
PERE [MJ] 3.81E+1 1.12E-1 3.50E+0 0.00E+0 2.75E+0 0.00E+0 6.17E-3 2.79E-1 4.18E-1 1.99E-1 -7.36E-1 0.00E+0 -2.48E+0-2.33E-1
PERM [MJ] 2.30E-2 0.00E+0 -2.30E-2 0.00E+0 0.00E+0 0.00E+0 0.00E+0 0.00E+0 0.00E+0 0.00E+0 0.00E+0 0.00E+0 0.00E+0 0.00E+0
PERT [MJ] 3.82E+1 1.12E-1 3.48E+0 0.00E+0 2.75E+0 0.00E+0 6.17E-3 2.79E-1 4.18E-1 1.99E-1 -7.36E-1 0.00E+0 -2.48E+0-2.33E-1
PENRE [MJ] 8.23E+1 1.97E+0 1.29E+1 0.00E+0 4.50E+0 0.00E+0 1.09E-1 2.04E+1 2.09E+1 2.42E+0 -2.69E+0 0.00E+0 -9.21E+0-1.72E+1
PENRM [MJ] 2.19E+1 0.00E+0 -3.18E+0 0.00E+0 0.00E+0 0.00E+0 0.00E+0 -1.87E+1-1.87E+1 0.00E+0 0.00E+0 0.00E+0 0.00E+0 0.00E+0
PENRT [MJ] 1.04E+2 1.97E+0 9.75E+0 0.00E+0 4.50E+0 0.00E+0 1.09E-1 1.70E+0 2.19E+0 2.42E+0 -2.69E+0 0.00E+0 -9.21E+0-1.72E+1
SM [kg] 7.19E-1 0.00E+0 6.47E-2 0.00E+0 0.00E+0 0.00E+0 0.00E+0 0.00E+0 0.00E+0 0.00E+0 0.00E+0 0.00E+0 0.00E+0 6.44E-1
RSF [MJ] 0.00E+0 0.00E+0 0.00E+0 0.00E+0 0.00E+0 0.00E+0 0.00E+0 0.00E+0 0.00E+0 0.00E+0 0.00E+0 0.00E+0 0.00E+0 0.00E+0
NRSF [MJ] 0.00E+0 0.00E+0 0.00E+0 0.00E+0 0.00E+0 0.00E+0 0.00E+0 0.00E+0 0.00E+0 0.00E+0 0.00E+0 0.00E+0 0.00E+0 0.00E+0
FW [m³] 1.03E-1 1.27E-4 1.07E-2 0.00E+0 2.52E-3 0.00E+0 6.98E-6 1.02E-2 1.03E-2 2.83E-5 -7.04E-4 0.00E+0 -2.37E-3 -1.62E-3
PERE = Use of renewable primary energy excluding renewable primary energy resources used as raw materials; PERM = Use of
renewable primary energy resources used as raw materials; PERT = Total use of renewable primary energy resources; PENRE = Use of
non-renewable primary energy excluding non-renewable primary energy resources used as raw materials; PENRM = Use of non-
Caption
renewable primary energy resources used as raw materials; PENRT = Total use of non-renewable primary energy resources; SM = Use
of secondary material; RSF = Use of renewable secondary fuels; NRSF = Use of non-renewable secondary fuels; FW = Use of net fresh
water
RESULTS OF THE LCA – WASTE CATEGORIES AND OUTPUT FLOWS according to EN 15804+A2:
1 m² floor covering
Indicator Unit A1-A3 A4 A5 B1 B2 C1 C2 C3/2 C3/3 C4/1 D D/1 D/2 D/3
HWD [kg] 1.95E-3 9.45E-12 1.76E-4 0.00E+0 2.56E-5 0.00E+0 5.21E-132.59E-102.80E-103.72E-10-3.65E-100.00E+0 -1.26E-9-1.25E-10
NHWD [kg] 4.21E-1 2.83E-4 8.71E-2 0.00E+0 5.14E-3 0.00E+0 1.56E-5 5.37E-1 5.37E-1 2.39E+0 -1.36E-3 0.00E+0 -4.61E-3 -7.19E-2
RWD [kg] 2.57E-3 2.43E-6 2.39E-4 0.00E+0 3.74E-4 0.00E+0 1.34E-7 6.12E-5 9.72E-5 2.97E-5 -2.11E-4 0.00E+0 -7.10E-4 -4.88E-5
CRU [kg] 0.00E+0 0.00E+0 0.00E+0 0.00E+0 0.00E+0 0.00E+0 0.00E+0 0.00E+0 0.00E+0 0.00E+0 0.00E+0 0.00E+0 0.00E+0 0.00E+0
MFR [kg] 1.31E-2 0.00E+0 1.32E-2 0.00E+0 0.00E+0 0.00E+0 0.00E+0 0.00E+0 6.44E-1 0.00E+0 0.00E+0 0.00E+0 0.00E+0 0.00E+0
MER [kg] 0.00E+0 0.00E+0 0.00E+0 0.00E+0 0.00E+0 0.00E+0 0.00E+0 0.00E+0 0.00E+0 0.00E+0 0.00E+0 0.00E+0 0.00E+0 0.00E+0
EEE [MJ] 0.00E+0 0.00E+0 9.84E-1 0.00E+0 0.00E+0 0.00E+0 0.00E+0 5.44E+0 0.00E+0 0.00E+0 0.00E+0 0.00E+0 0.00E+0 0.00E+0
EET [MJ] 0.00E+0 0.00E+0 1.77E+0 0.00E+0 0.00E+0 0.00E+0 0.00E+0 9.93E+0 3.95E+1 0.00E+0 0.00E+0 0.00E+0 0.00E+0 0.00E+0
HWD = Hazardous waste disposed; NHWD = Non-hazardous waste disposed; RWD = Radioactive waste disposed; CRU = Components
Caption for re-use; MFR = Materials for recycling; MER = Materials for energy recovery; EEE = Exported electrical energy; EET = Exported
thermal energy
RESULTS OF THE LCA – additional impact categories according to EN 15804+A2-optional:
1 m² floor covering
Indicator Unit A1-A3 A4 A5 B1 B2 C1 C2 C3/2 C3/3 C4/1 D D/1 D/2 D/3
[Disease
PM 1.05E-7 5.07E-9 1.12E-8 0.00E+0 4.27E-8 0.00E+02.79E-10 1.27E-8 1.36E-8 4.85E-9 -1.72E-9 0.00E+0 -5.83E-9 -1.49E-8
Incidence]
[kBq U235-
IRP 3.89E-1 3.56E-4 3.62E-2 0.00E+0 6.58E-2 0.00E+0 1.96E-5 9.37E-3 1.55E-2 4.38E-3 -3.57E-2 0.00E+0 -1.20E-1 -5.79E-3
Eq.]
ETP-fw [CTUe] 4.57E+1 1.37E+0 4.33E+0 3.60E-3 2.03E+0 0.00E+0 7.54E-2 8.04E-1 1.09E+0 2.36E+0 -5.89E-1 0.00E+0-1.98E+0-3.14E+0
-2.71E- -9.25E- -4.16E-
HTP-c [CTUh] 2.44E-9 2.76E-112.28E-100.00E+03.90E-100.00E+01.52E-124.19E-114.85E-111.06E-10 0.00E+0
11 11 11
HTP-nc [CTUh] 1.05E-7 1.64E-9 9.91E-9 2.60E-11 6.19E-9 0.00E+09.03E-11 2.54E-9 2.87E-9 8.89E-9 -1.04E-9 0.00E+0 -3.56E-9 -2.62E-9
SQP [-] ND ND ND ND ND ND ND ND ND ND ND ND ND ND
PM = Potential incidence of disease due to PM emissions; IR = Potential Human exposure efficiency relative to U235; ETP-fw = Potential
Caption comparative Toxic Unit for ecosystems; HTP-c = Potential comparative Toxic Unit for humans (cancerogenic); HTP-nc = Potential
comparative Toxic Unit for humans (not cancerogenic); SQP = Potential soil quality index
No substantiated values can be given for the SQP indicator with the existing database.
The result figures given in module B2 refer to a period of 1 year because a reference service life is not declared.
They have to be multiplied by the assumed service life (in years) of the floor covering in the building under
consideration.
Disclaimer 1 – for the indicator “Potential Human exposure efficiency relative to U235”.
This impact category deals mainly with the eventual impact of low dose ionizingradiation on human health of the
nuclear fuel cycle. It does not consider effects due to possible nuclear accidents, occupational exposure nor due
to radioactive waste disposal in undergroundfacilities. Potential ionizing radiation from the soil, from radon and
from some construction materials is also not measured by this indicator.
Disclaimer 2 – for the indicators “abiotic depletion potential for non-fossil resources”, “abiotic depletion potential
for fossil resources”, “water (user) deprivation potential, deprivation-weighted water consumption”, “potential
comparative toxic unit for ecosystems”, “potential comparative toxic unit for humans – cancerogenic”, “Potential
comparative toxic unit for humans - not cancerogenic”, “potential soil quality index”.
The results of this environmental impact indicator shall be used with care as the uncertainties on these results are
high or as there is limited experience with the indicator.
References
EN 1307 DIN EN ISO 14040:2006+A1:2020 Environmental
DIN EN 1307: 2014+A1:2016+A2:2018-05: Textile management - Life cycle assessment - Principles and
floor coverings - Classification framework
EN 13501-1 ISO 14044
DIN EN 13501-1:2019-05: Fire classification of DIN EN ISO 14044:2006+A1:2018+A2:2020
construction products and building elements - Part 1: Environmental management - Life cycle assessment -
Classification using data from reaction to fire tests Requirements and guidelines
EN 14041 ISO 15686
DIN EN 14041: 2018-05 and DIN EN 14041: 2008-05: ISO 15686: Buildings and constructed assets -
Resilient, textile and laminate floor coverings - Service life planning
Essential characteristics ISO 15686-1: 2011-05: Part 1: General principles and
framework
EN 15804 ISO 15686-2: 2012-05: Part 2: Service life prediction
DIN EN 15804:2012+A2:2019 + AC:2021, procedures
Sustainability of construction works — Environmental ISO 15686-7: 2017-04: Part 7: Performance
Product Declarations — Core rules for the product evaluation for feedback of service life data
category of construction products from practice
ISO 15686-8: 2008-06: Part 8: Reference service life
EN 16810 and service-life estimation
DIN EN 16810: 2017-08: Resilient, textile and laminate
floor coverings – Environmental product declarations – Regulation (EU) No. 305/2011
Product category rules Regulation No. 305/2011 Construction Products
Regulation (CPR) of the European Council and of the
ISO 10874 European Parliament, April 2011
DIN EN ISO 10874: 2012+A1:2021-04: Resilient,
textile and laminate floor coverings - Classification General Instructions for the IBU-EPD Program
General Instructions for the EPD-Program of the
ISO 14025 Institut Bauen und Umwelt e.V., The Preparation of
DIN EN /ISO 14025:2011-10/, Environmental labels Environmental Product Declarations - EPDs, version
and declarations — Type III environmental 2.0, Institut Bauen und Umwelt e.V., Berlin, January
declarations — Principles and procedures 2021, www.ibu-epd.de
ISO 14040
7 Environmental Product Declaration GUT e.V. – Tufted wall-to-wall carpet with 100% recycled PA6 pile material and textile
backing, LC1
BNB, Nutzungsdauer von Bauteilen Product Category Rules for Building-Related Products
Bewertungssystem Nachhaltiges Bauen (BNB), and Services
Nutzungsdauer von Bauteilen, Bundesministerium des Part B: Requirements on the EPD for floor coverings,
Inneren, für Bau und Heimat, 24.02.2017 V1.2, Berlin: Institut Bauen und Umwelt e.V. (IBU),
February 2018
ECHA candidate list
Candidate List of substances of very high concern PRODIS
(SVHCs) for authorisation, 08.07.2021, European Product Information System (PRODIS) of the
Chemicals Agency (ECHA), Helsinki, Finland European Carpet Industry, Gemeinschaft
umweltfreundlicher Teppichboden e.V (GUT) and
ecoinvent European Carpet and Rug Association
ecoinvent, Zurich, Switzerland, database version 3.7, (ECRA), http://www.pro-dis.info
published September 2020
REACH
GaBi database Regulation (EC) No 1907/2006 of the European
GaBi Software-System and Database for Life Cycle Parliament and of the Council of 18 December 2006
Engineering, thinkstep AG, Leinfelden-Echterdingen, concerning the Registration, Evaluation, Authorisation
2022-1 and Restriction of Chemicals (REACH), June 2017,
last update: 08.07.2021
PCR Part A
Product Category Rules for Building-Related Products VDZ e.V.
and Services Part A: Calculation Rules for the Life Association of German Cement Works, Ed. Environ-
Cycle Assessment and Requirements on the Project mental Data of the German Cement Industry 2020
Report according to EN 15804+A2:2019, V1.2, Berlin:
Institut Bauen und Umwelt e.V. (IBU), November 2021
PCR Part B
8 Environmental Product Declaration GUT e.V. – Tufted wall-to-wall carpet with 100% recycled PA6 pile material and textile
backing, LC1
Publisher
Institut Bauen und Umwelt e.V. Tel +49 (0)30 3087748- 0
Hegelplatz 1 Fax +49 (0)30 3087748- 29
10117 Berlin Mail info@ibu-epd.com
Germany Web www.ibu-epd.com
Programme holder
Institut Bauen und Umwelt e.V. Tel +49 (0)30 - 3087748- 0
Hegelplatz 1 Fax +49 (0)30 – 3087748 - 29
10117 Berlin Mail info@ibu-epd.com
Germany Web www.ibu-epd.com
Author of the Life Cycle
Assessment Tel +49 (0)241 96843 410
Gemeinschaft umweltfreundlicher Fax +49 (0)241 96843 400
Teppichboden (GUT) e.V. Mail mail@gut-ev.de
Schönebergstraße 2 Web www.gut-ev.org
52068 Aachen
Germany
Owner of the Declaration
Gemeinschaft umweltfreundlicher Tel +49 (0)241 96843 410
Teppichboden (GUT) e.V. Fax +49 (0)241 96843 400
Schönebergstraße 2 Mail mail@gut-ev.de
52068 Aachen Web www.gut-ev.org
Germany
