ENVIRONMENTAL PRODUCT DECLARATION
as per ISO 14025 and EN 15804+A2
Owner of the Declaration Milliken Industrials Ltd.
Programme holder Institut Bauen und Umwelt e.V. (IBU)
Publisher Institut Bauen und Umwelt e.V. (IBU)
Declaration number EPD-MIL-20230039-CBA1-EN
Issue date 20.02.2023
Valid to 19.02.2028
Tufted carpet tiles
pile material polyamide 6 with 100% recycled content,
maximum total pile weight 1010 g/m2, print design,
Comfort Lite®/Comfort Plus® recycled cushion back
Milliken
www.ibu-epd.com | https://epd-online.com
Umwelt Produktdeklaration Name des Herstellers – Name des Produkts
General Information
Milliken Tufted carpet tiles
pile material PA 6 with 100% recycled
content, max. total pile weight 1010
g/m2, print design, Comfort Lite®/
Comfort Plus® recycled cushion back
Programme holder Owner of the declaration
IBU – Institut Bauen und Umwelt e.V. Milliken Industrials Ltd.
Hegelplatz 1 Beech Hill Plant, Gidlow Lane
10117 Berlin Wigan WN6 8RN
Germany United Kingdom
Declaration number Declared product / declared unit
EPD-MIL-20230039-CBA1-EN 1 m2 tufted carpet tiles having a pile material of
polyamide 6 with 100% recycled content and a Comfort
Lite® or Comfort Plus® recycled cushion back.
This declaration is based on the product Scope:
category rules: The manufacturer declaration applies to a group of
Floor coverings, 09.2022 products with a maximum total pile weight of 1010
(PCR checked and approved by the SVR) g/m2. LCA results for products of the same
construction but with a maximum total pile weight of
400 g/m2 can be taken from the corresponding tables
Issue date
of the annexe. Specific data for every product within
20.02.2023
the declared group of products in relation to its total
pile weight can be calculated by using equation 1 given
Valid to in the annexe (see annexe chapter: 'General
19.02.2028 Information on the annexe').
The carpet is manufactured at the Milliken production
site in Wigan, United Kingdom.
The declaration is only valid in conjunction with a valid
GUT-PRODIS license of the product.
The owner of the declaration shall be liable for the
underlying information and evidence; the IBU shall not
be liable with respect to manufacturer information, life
cycle assessment data and evidences.
The EPD was created according to the specifications
of EN 15804+A2. In the following, the standard will be
simplified as EN 15804.
Verification
The standard EN 15804 serves as the core PCR
Independent verification of the declaration and data
according to ISO 14025:2011
Dipl. Ing. Hans Peters internally x externally
(chairman of Institut Bauen und Umwelt e.V.)
Dr. Alexander Röder Angela Schindler
(Managing Director Institut Bauen und Umwelt e.V.)) (Independent verifier)
Product
Product description/Product definition felt backing with recycled content.
Tufted carpet tiles having a pile material of polyamide The recycled content based on the total weight of the
6 with 100% recycled content and a Comfort Lite® or product amounts to 71%.
Comfort Plus® recycled cushion back. The injection The declaration applies to a group of products with a
printing system Millitron® allows the creation of various maximum total pile weight of 1010 g/m2.
designs. The LCA results are calculated for products with the
The bitumen based heavy backing with recycled filler maximum total pile weight. LCA results for products
includes a glass fibre reinforcement and a 90% with a maximum total pile weight of 400 g/m2 can be
recycled polyurethane cushion and it is covered with a taken from the corresponding tables of the annexe.
2 Environmental Product Declaration Milliken – Tufted carpet tiles, total pile material max. 1010 g/m² PA 6 with 100%
recycled content, print design, Comfort Lite®/Plus® recycled cushion back
Results for specific products with any other total pile Additional product properties in accordance with EN
weight can be calculated by using equation 1 given in 1307 can be found on the Product Information System
the annexe (see annexe chapter: 'General Information PRODIS using the PRODIS registration number of the
on the annexe'). product (www.pro-dis.info) or on the manufacturer's
For the placing on the market of the specific product in technical information section.
the European Union/European Free Trade Association
(EU/EFTA) (with the exception of Switzerland) Base materials/Ancillary materials
Regulation (EU) No. 305/2011 Construction Product
Regulation (CPR) applies. The product needs a Name Value Unit
Declaration of Performance (DoP) taking into Polyamide 6 21.0 %
consideration EN 14041:2018-05, Resilient, textile and Polyester 4.5 %
laminate floor coverings - Essential characteristics, and Polypropylene 1.1 %
the CE-marking. The DoP of the product can be found Limestone 36.5 %
on the manufacturer's technical information section. Bitumen 10.5 %
For the application and use of the product the Aluminum hydroxide 8.6 %
respective national provisions apply. Ethyl vinyl acetate 3.5 %
Glass fibre 0.9 %
Application
Polyurethane 12.9 %
According to the use class as defined in EN 1307 the
Additives 0.5 %
products can be used in all professional area with
heavy use which require class 33 or less.
The specific product coverd by the EPD contains
substances listed in the ECHA candidate list
(26.07.2022) or other carcinogenic, mutagenic or
reprotoxic (CMR) substances in categories 1A or 1B
which are not on the candidate list exceeding 0.1
percentage by mass: no
Technical Data The products are registered in the GUT-PRODIS
Information System. The PRODIS system ensures the
compliance with limitations of various chemicals and
Constructional data according to EN 1307 Volatile Organic Compound (VOC)-emissions and a
Name Value Unit ban on the use of all substances that are listed as
Tiles or modules, 'Substances of Very High Concern' (SVHC) under
Product Form -
several dimensions REACH.
Type of
Tufted carpet -
manufacture Reference service life
Colouration Injection print design - The service life of textile floor coverings strongly
Polyamide 6 with depends on the correct installation taking into account
Yarn type -
100% recycled content the declared use classification and the adherence to
Comfort Lite®/Comfort Plus® cleaning and maintenance instructions.
Secondary backing -
recycled cushion back A calculation of the reference service life according to
Total pile weight max. 1010 g/m² ISO 15686 is not possible.
Total carpet weight max. 4800 g/m2 Alternatively, a reference service life of 10 years can
be assumed, during which the functional and visual
quality is guaranteed (BNB, Nutzungsdauer von
Performance data of the product in accordance with Bauteilen). The technical service life can be
the declaration of performance with respect to its significantly longer.
essential characteristics according to EN 14041: 2018-
05, Resilient, textile and laminate floor coverings -
Essential characteristics.
LCA: Calculation rules
Declared Unit number of the product (www.pro-dis.info) or on the
manufacturer's technical information section.
Name Value Unit
Declared unit 1 m2 System boundary
Grammage 4.8 kg/m2
Layer thickness (average value for Type of EPD:
0.011 m
the tiles) Cradle-to-gate with options, module C1-C4, module D,
Gross density (average value for and additional modules A4, A5, B1, B2.
440 kg/m3
the tiles)
The declared unit refers to 1 m2 produced textile floor System boundaries of modules A, B, C, D:
covering. The Output of module A5 'Assembly' is 1 m2 Modules C3, C4 and D are indicated separately for
installed textile floor covering. three end-of-life scenarios:
The layer thickness of the specific product covered by 1 - landfill disposal
the EPD can be found on the Product Information 2 - municipal waste incineration
System PRODIS using the PRODIS registration 3 - recovery in a cement plant
3 Environmental Product Declaration Milliken – Tufted carpet tiles, total pile material max. 1010 g/m² PA 6 with 100%
recycled content, print design, Comfort Lite®/Plus® recycled cushion back
B6 - B7:
A1-A3 Production: No energy and water input are required for the
Energy supply and production of the basic material, operation of the carpet in the use stage. The modules
processing of secondary material, auxiliary material, are not relevant and not declared.
transport of the material to the manufacturing site,
emissions, waste water treatment, packaging material C1 De-construction:
and waste processing up to the landfill disposal of The floor covering is de-constructed manually and no
residual waste (except radioactive waste). Benefits for additional environmental impact is caused.
generated electricity and steam due to the incineration
of production waste are aggregated. C2 Transport:
Biogenic carbon that is stored in renewable material Transport of the carpet waste to a landfill, to the
(packaging paper) is taken into account as well as the municipal waste incineration plant (MWI) or to the
associated uptake of carbon dioxide from the air from waste collection facility for recycling.
which this biogenic carbon originates.
C3 Waste processing:
A4 Transport: C3-1: Landfill disposal needs no waste processing.
Transport of the packed textile floor covering from C3-2: Impact from waste incineration (plant with
factory gate to the place of installation. R1>0.6), generated electricity and steam are listed in
the result table as exported energy.
A5 Installation: C3-3: Collection of the carpet waste for recovery in the
Installation of the textile floor covering, processing of cement industry, waste processing (granulating),
installation waste and packaging waste up to the transport to the cement plant, emissions from the
landfill disposal of residual waste (except radioactive incineration. The biogenic carbon that is stored in the
waste), the production of the amount of carpet that renewable materials of the floor covering is released
occurs as installation waste including its transport to into the air as carbon dioxide emissions.
the place of installation.
Generated electricity and steam due to the incineration C4 Disposal:
of waste are listed in the result table as exported C4-1: Impact from landfill disposal,
energy. C4-2: The carpet waste leaves the system in
Biogenic carbon stored in renewable materials in module C3-2,
packaging paper is released into the air as carbon C4-3: The pre-processed carpet waste leaves the
dioxide emissions at the end of the life cycle in module system in module C3-3.
A5.
Preparation of the floor and auxiliary materials D Recycling potential:
(adhesives, fixing agents, PET connectors) are beyond Calculated benefits result from materials exclusive
the system boundaries and not taken into account. secondary materials (net materials).
D-A5: Benefits for generated energy due to
B1 Use: incineration of packaging and installation waste
Indoor emissions during the use stage. After the first (incineration plant with R1 > 0.6),
year, no product-related Volatile Organic Compound D-1: Benefits for generated energy due to landfill
(VOC) emissions are relevant due to known VOC disposal of carpet waste at the end of life,
decay curves of the product. D-2: Benefits for generated energy due to incineration
of carpet waste at the end-of-life (incineration plant
B2 Maintenance: with R1 > 0.6),
Cleaning of the textile floor covering for a period of 1 D-3: Benefits for saved fossil energy and saved
year: inorganic material due to recovery of the carpet in a
Vacuum cleaning – electricity supply cement plant.
Wet cleaning – electricity, water consumption,
production of the cleaning agent, waste water Comparability
treatment. Basically, a comparison or an evaluation of EPD data
The declared values in this module have to be is only possible if all the data sets to be compared
multiplied by the assumed service life of the floor were created according to EN 15804 and the building
covering in the building in question. context, respectively the product-specific
characteristics of performance, are taken into account.
B3 - B5:
The modules are not relevant within the assumed Background data are taken from the GaBi database,
reference service life of 10 years. 2022-2.
LCA: Scenarios and additional technical information
Characteristic product properties
Information on biogenic carbon Information on describing the biogenic Carbon
The following information refer to the declared modules Content at factory gate
and are the basis for calculations or can be used for Name Value Unit
further calculations. The indicated values refer to the Biogenic carbon content in
declared functional unit of all products with a max. total accompanying packaging at 0.086 kg C
pile weight of 1010 g/m2. factory gate
1 kg biogenic Carbon is equivalent to 44/12 kg of CO
2
4 Environmental Product Declaration Milliken – Tufted carpet tiles, total pile material max. 1010 g/m² PA 6 with 100%
recycled content, print design, Comfort Lite®/Plus® recycled cushion back
Transport to the construction site (A4)
Name Value Unit If combinations of these scenarios have to be
Litres of fuel (truck, EURO 0-6 mix) 0.0113 l/100km calculated this should be done according to the
Transport distance 700 km following scheme:
Capacity utilisation (including empty EOL-impact = x % impact (Scenario 1)
55 %
runs) + y % impact (Scenario 2)
+ z % impact (Scenario 3)
Installation in the building (A5) with x % + y % + z % = 100 %
Name Value Unit
Material loss 0.144 kg Name Value Unit
Polyethylene packaging waste and installation waste Collected as mixed construction waste
4.8 kg
are considered to be incinerated in a municipal waste (scenarios 1 and 2)
incineration plant. Cardboard packaging waste is Collected separately (scenario 3) 4.8 kg
recycled. Landfilling (scenario 1) 4.8 kg
Preparation of the floor and auxiliaries (adhesives, Energy recovery (scenario 2) 4.8 kg
fixing agents, PET connectors etc.) are not taken into Energy recovery (scenario 3) 2.59 kg
account. Recycling (scenario 3) 2.21 kg
Maintenance (B2) Reuse, recovery and/or recycling potentials (D),
The values for cleaning refer to 1 m2 floor covering per relevant scenario information
year. Recovery or recycling potentials due to the three end-
Depending on the application based on ISO 10874, the of-life scenarios (module C) are indicated separately.
technical service life recommended by the
manufacturer and the anticipated strain on the floor by Recycling in the cement industry (scenario 3)
customers, the case-specific useful life can be The organic material of the carpet is used as an
established. Based on this useful life the effects of alternative fuel in a cement kiln. It mainly substitutes
module B2 need to be calculated in order to obtain the for lignite (68.8 %), hard coal (23.6 %) and petrol coke
overall environmental impacts. (7.6 %). The inorganic material is substantially
integrated into the cement clinker and substitutes for
Name Value Unit original material input. VDZ e.V.
Number
Maintenance cycle (vacuum cleaning) 208
/year
Number
Maintenance cycle (wet cleaning) 1,5
/year
Water consumption (wet cleaning) 0.004 m3
Cleaning agent (wet cleaning) 0.09 kg
Electricity consumption 0.314 kWh
For further information on cleaning and maintenance
see www.millikencarpet.com
Service life
Name Value Unit
Life Span (according to
10 a
BBSR)
Declared product Corresponds to the
properties (at the gate) and specifications of -
finishes EN 1307
An assumed quality of
Conforms to the
work, when installed in
manufacturer's -
accordance with the
instructions
manufacturer’s instructions
Usage conditions, e.g. Use in areas defined by
frequency of use, the use class according -
mechanical exposure to EN 1307
Maintenance e.g. required
According to the
frequency, type and quality
manufacturers -
and replacement of
instructions
components
End of Life (C1-C4)
Three different end-of-life scenarios are declared and
the results are indicated separately in module C.
Each scenario is calculated as a 100% scenario.
Scenario 1: 100 % landfill disposal
Scenario 2: 100 % municipal waste incineration (MWI)
with R1>0.6
Scenario 3: 100 % recovery in the cement industry
5 Environmental Product Declaration Milliken – Tufted carpet tiles, total pile material max. 1010 g/m² PA 6 with 100%
recycled content, print design, Comfort Lite®/Plus® recycled cushion back
LCA: Results
The LCA results refer to all declared products with a maximum total pile weight of 1010 g/m2. LCA results for
products with a maximum total pile weight of 400 g/m2 can be taken from the corresponding tables of the annexe.
Results for specific products with any other total pile weight can be calculated by using equation 1 given in the
annexe (see annexe chapter: 'General Information on the annexe').
The declared result figures in module B2 have to be multiplied by the assumed service life (in years) of the floor
covering in the building under consideration.
Information on non-relevant modules:
Modules B3 - B7 are not relevant during the service life of the carpet.
Modules C3/1, C4/2 and C4/3 cause no additional impact (see chapter "LCA: Calculation rules" in this document).
Module C2 represents the transport for scenarios 1, 2 and 3. The values in column D result from module A5.
DESCRIPTION OF THE SYSTEM BOUNDARY (X = INCLUDED IN LCA; ND = MODULE OR INDICATOR NOT
DECLARED; MNR = MODULE NOT RELEVANT)
BENEFITS AND
CONSTRUCTI LOADS
PRODUCT STAGE ON PROCESS USE STAGE END OF LIFE STAGE BEYOND THE
STAGE SYSTEM
BOUNDARIES
6 Environmental Product Declaration Milliken – Tufted carpet tiles, total pile material max. 1010 g/m² PA 6 with 100%
recycled content, print design, Comfort Lite®/Plus® recycled cushion back
lairetam
waR
ylppus tropsnarT
gnirutcafunaM
eht
morf
tropsnarT
etis
eht
ot
etag
ylbmessA esU
ecnanetniaM
riapeR
tnemecalpeR tnemhsibrufeR
ygrene
lanoitarepO esu
retaw
lanoitarepO esu
noitcurtsnoc-eD
noitilomed tropsnarT
gnissecorp
etsaW
lasopsiD -esueR -yrevoceR -gnilcyceR laitnetop
A1 A2 A3 A4 A5 B1 B2 B3 B4 B5 B6 B7 C1 C2 C3 C4 D
X X X X X X X MNR MNR MNR ND ND X X X X X
RESULTS OF THE LCA - ENVIRONMENTAL IMPACT according to EN 15804+A2: 1 m² floor covering
Core Indicator Unit A1-A3 A4 A5 B1 B2 C1 C2 C3/2 C3/3 C4/1 D D/1 D/2 D/3
GWP-total [kg CO2-Eq.] 5.71E+02.97E-1 6.88E-10.00E+05.49E-10.00E+01.63E-26.08E+06.15E+03.37E-1-2.02E-20.00E+0-4.24E-1-3.17E-1
GWP-fossil [kg CO2-Eq.] 5.99E+02.92E-1 3.87E-10.00E+03.48E-10.00E+01.60E-26.08E+06.15E+03.37E-1-2.01E-20.00E+0-4.22E-1-3.16E-1
GWP-biogenic [kg CO2-Eq.] -3.29E-13.78E-3 2.99E-10.00E+04.16E-30.00E+02.07E-4 7.77E-4 1.52E-3-5.53E-8-1.02E-40.00E+0-2.13E-3-5.90E-4
GWP-luluc [kg CO2-Eq.] 4.73E-2 1.65E-3 1.48E-30.00E+01.96E-10.00E+09.06E-5 2.32E-4 4.64E-4 1.66E-4-2.18E-60.00E+0-4.55E-5-1.59E-4
1.78E- 3.70E- 9.73E- 5.18E- 8.81E- 4.57E- -1.34E- -2.79E- -3.47E-
ODP [kg CFC11-Eq.] 1.23E-8 0.00E+03.42E-80.00E+0 0.00E+0
14 10 16 13 13 13 13 12 13
AP [mol H+-Eq.] 1.78E-2 1.76E-3 7.68E-40.00E+08.32E-40.00E+09.67E-5 5.84E-3 6.14E-3 1.01E-3-2.62E-50.00E+0-5.48E-4-1.30E-3
EP-freshwater [kg P-Eq.] 7.78E-5 8.84E-7 2.39E-60.00E+05.19E-60.00E+04.85E-8 8.48E-7 1.04E-6 6.35E-5-2.72E-80.00E+0-5.67E-7-3.48E-7
EP-marine [kg N-Eq.] 6.22E-3 8.66E-4 3.01E-40.00E+01.97E-40.00E+04.75E-5 2.86E-3 2.99E-3 2.23E-4-7.12E-60.00E+0-1.49E-4-3.80E-4
EP-terrestrial [mol N-Eq.] 5.67E-2 9.59E-3 2.98E-30.00E+02.83E-30.00E+05.26E-4 3.20E-2 3.34E-2 2.45E-3-7.63E-50.00E+0-1.60E-3-4.16E-3
POCP [kg NMVOC-Eq.]1.55E-2 1.64E-3 7.41E-4 4.18E-4 9.83E-40.00E+08.98E-5 7.34E-3 7.59E-3 7.18E-4-2.00E-50.00E+0-4.19E-4-1.12E-3
ADPE [kg Sb-Eq.] 3.12E-6 2.48E-8 9.54E-80.00E+02.30E-70.00E+01.36E-9 2.84E-8 3.85E-8 2.36E-8-3.00E-90.00E+0-6.26E-8-3.11E-8
- -
ADPF [MJ] 1.20E+23.96E+03.83E+00.00E+05.90E+00.00E+02.17E-13.39E+04.38E+04.83E+0-3.41E-10.00E+0
7.17E+03.18E+1
[m³ world-Eq
WDP 4.21E+02.65E-3 1.52E-10.00E+09.99E-20.00E+01.45E-4 8.02E-1 8.08E-1-3.61E-3-2.09E-30.00E+0-4.34E-2-4.40E-2
deprived]
GWP = Global warming potential; ODP = Depletion potential of the stratospheric ozone layer; AP = Acidification potential of land and water; EP =
Caption Eutrophication potential; POCP = Formation potential of tropospheric ozone photochemical oxidants; ADPE = Abiotic depletion potential for non-
fossil resources; ADPF = Abiotic depletion potential for fossil resources; WDP = Water (user) deprivation potential
RESULTS OF THE LCA - INDICATORS TO DESCRIBE RESOURCE USE according to EN 15804+A2: 1 m²
floor covering
Indicator Unit A1-A3 A4 A5 B1 B2 C1 C2 C3/2 C3/3 C4/1 D D/1 D/2 D/3
PERE [MJ] 8.78E+1 2.25E-1 3.23E+0 0.00E+0 3.69E+0 0.00E+0 1.23E-2 5.66E-1 8.44E-1 3.97E-1 -9.24E-2 0.00E+0 -1.92E+0-4.83E-1
PERM [MJ] 5.52E-1 0.00E+0 -5.52E-1 0.00E+0 0.00E+0 0.00E+0 0.00E+0 0.00E+0 0.00E+0 0.00E+0 0.00E+0 0.00E+0 0.00E+0 0.00E+0
PERT [MJ] 8.83E+1 2.25E-1 2.67E+0 0.00E+0 3.69E+0 0.00E+0 1.23E-2 5.66E-1 8.44E-1 3.97E-1 -9.24E-2 0.00E+0 -1.92E+0-4.83E-1
PENRE [MJ] 8.58E+1 3.97E+0 4.05E+0 0.00E+0 5.90E+0 0.00E+0 2.18E-1 3.75E+1 3.84E+1 4.83E+0 -3.41E-1 0.00E+0 -7.17E+0-3.18E+1
PENRM [MJ] 3.43E+1 0.00E+0 -2.15E-1 0.00E+0 0.00E+0 0.00E+0 0.00E+0 -3.41E+1-3.41E+1 0.00E+0 0.00E+0 0.00E+0 0.00E+0 0.00E+0
PENRT [MJ] 1.20E+2 3.97E+0 3.84E+0 0.00E+0 5.90E+0 0.00E+0 2.18E-1 3.39E+0 4.38E+0 4.83E+0 -3.41E-1 0.00E+0 -7.17E+0-3.18E+1
SM [kg] 1.85E+0 0.00E+0 5.55E-2 0.00E+0 0.00E+0 0.00E+0 0.00E+0 0.00E+0 0.00E+0 0.00E+0 0.00E+0 0.00E+0 0.00E+0 3.20E-1
RSF [MJ] 0.00E+0 0.00E+0 0.00E+0 0.00E+0 0.00E+0 0.00E+0 0.00E+0 0.00E+0 0.00E+0 0.00E+0 0.00E+0 0.00E+0 0.00E+0 0.00E+0
NRSF [MJ] 0.00E+0 0.00E+0 0.00E+0 0.00E+0 0.00E+0 0.00E+0 0.00E+0 0.00E+0 0.00E+0 0.00E+0 0.00E+0 0.00E+0 0.00E+0 0.00E+0
FW [m³] 1.21E-1 2.54E-4 4.25E-3 0.00E+0 3.34E-3 0.00E+0 1.40E-5 1.90E-2 1.92E-2 5.65E-5 -8.83E-5 0.00E+0 -1.84E-3 -3.10E-3
PERE = Use of renewable primary energy excluding renewable primary energy resources used as raw materials; PERM = Use of
renewable primary energy resources used as raw materials; PERT = Total use of renewable primary energy resources; PENRE = Use of
non-renewable primary energy excluding non-renewable primary energy resources used as raw materials; PENRM = Use of non-
Caption
renewable primary energy resources used as raw materials; PENRT = Total use of non-renewable primary energy resources; SM = Use
of secondary material; RSF = Use of renewable secondary fuels; NRSF = Use of non-renewable secondary fuels; FW = Use of net fresh
water
RESULTS OF THE LCA – WASTE CATEGORIES AND OUTPUT FLOWS according to EN 15804+A2:
1 m² floor covering
Indicator Unit A1-A3 A4 A5 B1 B2 C1 C2 C3/2 C3/3 C4/1 D D/1 D/2 D/3
HWD [kg] 2.83E-3 1.90E-11 8.49E-5 0.00E+0 4.19E-5 0.00E+0 1.04E-125.09E-105.50E-107.45E-10-4.63E-110.00E+0-9.78E-10-3.15E-10
NHWD [kg] 6.66E-1 5.69E-4 5.42E-2 0.00E+0 7.30E-3 0.00E+0 3.12E-5 1.14E+0 1.14E+0 4.78E+0 -1.71E-4 0.00E+0 -3.58E-3 -1.97E-1
RWD [kg] 1.57E-3 4.89E-6 5.11E-5 0.00E+0 3.76E-4 0.00E+0 2.68E-7 1.23E-4 1.95E-4 5.93E-5 -2.65E-5 0.00E+0 -5.52E-4 -1.08E-4
CRU [kg] 0.00E+0 0.00E+0 0.00E+0 0.00E+0 0.00E+0 0.00E+0 0.00E+0 0.00E+0 0.00E+0 0.00E+0 0.00E+0 0.00E+0 0.00E+0 0.00E+0
MFR [kg] 0.00E+0 0.00E+0 1.97E-1 0.00E+0 0.00E+0 0.00E+0 0.00E+0 0.00E+0 1.30E+0 0.00E+0 0.00E+0 0.00E+0 0.00E+0 0.00E+0
MER [kg] 0.00E+0 0.00E+0 0.00E+0 0.00E+0 0.00E+0 0.00E+0 0.00E+0 0.00E+0 0.00E+0 0.00E+0 0.00E+0 0.00E+0 0.00E+0 0.00E+0
EEE [MJ] 0.00E+0 0.00E+0 2.86E-1 0.00E+0 0.00E+0 0.00E+0 0.00E+0 8.41E+0 0.00E+0 0.00E+0 0.00E+0 0.00E+0 0.00E+0 0.00E+0
EET [MJ] 0.00E+0 0.00E+0 5.26E-1 0.00E+0 0.00E+0 0.00E+0 0.00E+0 1.55E+1 8.32E+1 0.00E+0 0.00E+0 0.00E+0 0.00E+0 0.00E+0
HWD = Hazardous waste disposed; NHWD = Non-hazardous waste disposed; RWD = Radioactive waste disposed; CRU = Components
Caption for re-use; MFR = Materials for recycling; MER = Materials for energy recovery; EEE = Exported electrical energy; EET = Exported
thermal energy
RESULTS OF THE LCA – additional impact categories according to EN 15804+A2-optional:
1 m² floor covering
Indicator Unit A1-A3 A4 A5 B1 B2 C1 C2 C3/2 C3/3 C4/1 D D/1 D/2 D/3
[Disease -2.17E-
PM 1.52E-7 1.02E-8 5.66E-9 0.00E+0 6.84E-8 0.00E+05.59E-10 2.52E-8 2.70E-8 9.69E-9 0.00E+0 0.00E+0 -1.83E-8
Incidence] 10
[kBq U235-
IRP 2.42E-1 7.16E-4 7.87E-3 0.00E+0 6.78E-2 0.00E+0 3.93E-5 1.88E-2 3.10E-2 8.76E-3 -4.49E-3 0.00E+0 0.00E+0 -1.36E-2
Eq.]
ETP-fw [CTUe] 5.69E+1 2.75E+0 1.85E+0 3.60E-3 2.69E+0 0.00E+0 1.51E-1 1.65E+0 2.22E+0 4.72E+0 -7.39E-2 0.00E+0 0.00E+0-5.97E+0
-3.43E- -8.86E-
HTP-c [CTUh] 2.68E-9 5.56E-118.48E-110.00E+06.21E-100.00E+03.05E-128.30E-119.63E-112.12E-10 0.00E+0 0.00E+0
12 11
-1.32E-
HTP-nc [CTUh] 8.05E-8 3.30E-9 2.69E-9 2.60E-11 9.46E-9 0.00E+01.81E-10 5.52E-9 6.17E-9 1.78E-8 0.00E+0 0.00E+0 -5.76E-9
10
SQP [-] ND ND ND ND ND ND ND ND ND ND ND ND ND ND
PM = Potential incidence of disease due to PM emissions; IR = Potential Human exposure efficiency relative to U235; ETP-fw = Potential
Caption comparative Toxic Unit for ecosystems; HTP-c = Potential comparative Toxic Unit for humans (cancerogenic); HTP-nc = Potential
comparative Toxic Unit for humans (not cancerogenic); SQP = Potential soil quality index
The SQP indicator is not given due to considerable uncertainties in the calculation.
The result figures given in module B2 refer to a period of 1 year because a reference service life is not declared.
They have to be multiplied by the assumed service life (in years) of the floor covering in the building under
consideration.
Disclaimer 1 – for the indicator “Potential Human exposure efficiency relative to U235”.
This impact category deals mainly with the eventual impact of low dose ionizing radiation on human health of the
nuclear fuel cycle. It does not consider effects due to possible nuclear accidents, occupational exposure or
radioactive waste disposal in underground facilities. Potential ionizing radiation from the soil, from radon and from
some construction materials is also not measured by this indicator.
Disclaimer 2 – for the indicators “abiotic depletion potential for non-fossil resources”, “abiotic depletion potential
for fossil resources”, “water (user) deprivation potential, deprivation-weighted water consumption”, “potential
comparative toxic unit for ecosystems”, “potential comparative toxic unit for humans – cancerogenic”, “Potential
comparative toxic unit for humans - not cancerogenic”, “potential soil quality index”.
The results of this environmental impact indicator shall be used with care as the uncertainties on these results are
high as there is limited experienced with the indicator.
References
EN 1307 EN 16810
DIN EN 1307: 2014+A1:2016+A2:2018-05: Textile DIN EN 16810: 2017-08: Resilient, textile and laminate
floor coverings - Classification floor coverings – Environmental product declarations –
Product category rules
EN 13501-1
DIN EN 13501-1:2019-05: Fire classification of ISO 10874
construction products and building elements - Part 1: DIN EN ISO 10874: 2012+A1:2021-04: Resilient,
Classification using data from reaction to fire tests textile and laminate floor coverings - Classification
EN 14041 ISO 14025
DIN EN 14041: 2018-05 and DIN EN 14041: 2008-05: DIN EN /ISO 14025:2011-10/, Environmental labels
Resilient, textile and laminate floor coverings - and declarations — Type III environmental
Essential characteristics declarations — Principles and procedures
EN 15804 ISO 14040
DIN EN 15804:2012+A2:2019 + AC:2021, DIN EN ISO 14040:2006+A1:2020 Environmental
Sustainability of construction works — Environmental management - Life cycle assessment - Principles and
Product Declarations — Core rules for the product framework
category of construction products
7 Environmental Product Declaration Milliken – Tufted carpet tiles, total pile material max. 1010 g/m² PA 6 with 100%
recycled content, print design, Comfort Lite®/Plus® recycled cushion back
ISO 14044
DIN EN ISO 14044:2006+A1:2018+A2:2020 ecoinvent
Environmental management - Life cycle assessment - ecoinvent, Zurich, Switzerland, database version 3.7,
Requirements and guidelines published September 2020
ISO 15686 GaBi database
ISO 15686: Buildings and constructed assets - GaBi Software-System and Database for Life Cycle
Service life planning Engineering, thinkstep AG, Leinfelden-Echterdingen,
ISO 15686-1: 2011-05: Part 1: General principles and 2022-2
framework
ISO 15686-2: 2012-05: Part 2: Service life prediction PCR Part A
procedures Product Category Rules for Building-Related Products
ISO 15686-7: 2017-04: Part 7: Performance and Services Part A: Calculation Rules for the Life
evaluation for feedback of service life data Cycle Assessment and Requirements on the Project
from practice Report according to EN 15804+A2:2019, V1.3, Berlin:
ISO 15686-8: 2008-06: Part 8: Reference service life Institut Bauen und Umwelt e.V. (IBU), August 2022
and service-life estimation
PCR Part B
Regulation (EU) No. 305/2011 Product Category Rules for Building-Related Products
Regulation No. 305/2011 Construction Products and Services
Regulation (CPR) of the European Council and of the Part B: Requirements on the EPD for floor coverings,
European Parliament, April 2011 V1.3, Berlin: Institut Bauen und Umwelt e.V. (IBU),
September 2022
General Instructions for the IBU-EPD Program
General Instructions for the EPD-Program of the PRODIS
Institut Bauen und Umwelt e.V., The Preparation of Product Information System (PRODIS) of the
Environmental Product Declarations - EPDs, version European Carpet Industry, Gemeinschaft
2.0, Institut Bauen und Umwelt e.V., Berlin, January umweltfreundlicher Teppichboden e.V (GUT) and
2021, www.ibu-epd.de European Carpet and Rug Association
(ECRA), http://www.pro-dis.info
BBSR
Bundesinstitut für Bau-, Stadt- und Raumforschung REACH
(BBSR) im Bundesamt für Bauwesen und Regulation (EC) No 1907/2006 of the European
Raumordnung (BBR), Bonn Parliament and of the Council of 18 December 2006
concerning the Registration, Evaluation, Authorisation
BNB, Nutzungsdauer von Bauteilen and Restriction of Chemicals (REACH), June 2017
Bewertungssystem Nachhaltiges Bauen (BNB),
Nutzungsdauer von Bauteilen, Bundesministerium des VDZ e.V.
Inneren, für Bau und Heimat, 24.02.2017 Association of German Cement Works, Ed. Environ-
mental Data of the German Cement Industry 2020
ECHA candidate list
Candidate List of substances of very high concern
(SVHCs) for authorisation, last update 26.07.2022,
European Chemicals Agency (ECHA), Helsinki,
Finland
8 Environmental Product Declaration Milliken – Tufted carpet tiles, total pile material max. 1010 g/m² PA 6 with 100%
recycled content, print design, Comfort Lite®/Plus® recycled cushion back
Publisher
Institut Bauen und Umwelt e.V. Tel +49 (0)30 3087748- 0
Hegelplatz 1 Fax +49 (0)30 3087748- 29
10117 Berlin Mail info@ibu-epd.com
Germany Web www.ibu-epd.com
Programme holder
Institut Bauen und Umwelt e.V. Tel +49 (0)30 - 3087748- 0
Hegelplatz 1 Fax +49 (0)30 – 3087748 - 29
10117 Berlin Mail info@ibu-epd.com
Germany Web www.ibu-epd.com
Author of the Life Cycle
Assessment Tel +49 (0)241 96843 410
Gemeinschaft umweltfreundlicher Fax +49 (0)241 96843 400
Teppichboden (GUT) e.V. Mail mail@gut-ev.de
Schönebergstraße 2 Web www.gut-ev.org
52068 Aachen
Germany
Owner of the Declaration
Milliken Industrials Ltd. Tel +44 (0) 1942 612777
Beech Hill Plant Fax .
Gidlow Lane Mail carpetenquiries@milliken.com
United Kingdom Web www.millikencarpet.com
