ENVIRONMENTAL
as per ISO 14025 and EN 15804+A2
Owner of the Declaration modulyss®
Programme holder Institut Bauen und Umwelt e.V. (IBU)
Publisher Institut Bauen und Umwelt e.V. (IBU)
Declaration number EPD-MOD-20220308-CBA1-EN
Issue date 10.01.2023
Valid to 09.01.2028
Modular carpet tiles
Pile material: polyamide 6 yarn from 100% recycled material
with a maximum total pile weight of 1300 g/m2
Back2Back or Comfortback
modulyss®
www.ibu-epd.com | https://epd-online.com
Umwelt Produktdeklaration Name des Herstellers – Name des Produkts
General Information
modulyss® Modular carpet tiles
Pile material: polyamide 6 yarn from
100% recycled material with a
maximum total pile weight of 1300
g/m2
Back2Back or Comfortback
Programme holder Owner of the declaration
IBU – Institut Bauen und Umwelt e.V. modulyss
Hegelplatz 1 Zevensterrestraat 21
10117 Berlin 9240 Zele
Germany Belgium
Declaration number Declared product / declared unit
EPD-MOD-20220308-CBA1-EN 1 m² tufted modular carpet tiles with PET felt covered
bitumen heavy backing and a pile material of PA 6 with
100 % recycled content
This declaration is based on the product Scope:
category rules: The manufacturer declaration applies to tufted carpet
Floor coverings, 02.2018 tiles with a bitumen heavy backing, a pile material of
(PCR checked and approved by the SVR) 100 % recycled PA 6 with a maximum total pile weight
of 1300 g/m2. The products are produced in Zele,
Belgium.
Issue date
LCA results for products with a maximum total pile
10.01.2023
weight of 480 g/m2 can be taken from the
corresponding tables of the annexe. Specific data for
Valid to every product within the declared group of products in
09.01.2028 relation to its total pile weight can be calculated by
using equation 1 given in the annexe (see annexe
chapter: 'General Information on the annexe'). The
declaration is only valid in conjunction with a valid
GUT-PRODIS license of the product.
The owner of the declaration shall be liable for the
underlying information and evidence; the IBU shall not
be liable with respect to manufacturer information, life
cycle assessment data and evidences.
The EPD was created according to the specifications
of EN 15804+A2. In the following, the standard will be
simplified as EN 15804.
Verification
The standard EN 15804 serves as the core PCR
Independent verification of the declaration and data
according to ISO 14025:2011
Dipl. Ing. Hans Peters internally x externally
(chairman of Institut Bauen und Umwelt e.V.)
Dr. Alexander Röder Angela Schindler
(Managing Director Institut Bauen und Umwelt e.V.)) (Independent verifier)
Product
Product description/Product definition covered by a PET fleece. The maximum total recycled
The declaration applies to tufted carpet tiles having a content is 74 %.
surface pile of 100 % recycled dyed polyamide 6 with a For the placing on the market of the specific product in
maximum total pile weight of 1300 g/m2. Colouring of the European Union/European Free Trade Association
the surface is achieved either by solution-dyed yarns (EU/EFTA) (with the exception of Switzerland)
or aqueous dyeing methods. The backing of the carpet Regulation (EU) No. 305/2011 Construction Product
consists of a bitumen heavy backing. In the Regulation (CPR) applies. The product needs a
comfortback range, the bitumen heavy backing is Declaration of Performance (DoP) taking into
2 Environmental Product Declaration modulyss – Tufted tiles, 100% recycled polyamide 6 with a maximum total pile weight
of 1300 g/m2 back2back or comfortback backing
consideration EN 14041:2018-05, Resilient, textile and Limestone 41.1 %
laminate floor coverings - Essential characteristics, and Aluminiumhydroxide 5.3 %
the CE-marking. The DoP of the product can be found Styrene butadiene rubber (SBR) 4.6 %
on the manufacturer's technical information section. SBS Copolymer 1.0 %
For the application and use of the product the Bitumen 11.3 %
respective national provisions apply. Glass fibre 0.2 %
Additives 0.9 %
Application
The use class of the specific product as defined in
The specific product covered by the EPD contains
EN 1307 can be found in the Product Information
substances listed in the ECHA candidate list
System (PRODIS) using the PRODIS registration
(08.07.2021) or other carcinogenic, mutagenic or
number of the product.
reprotoxic (CMR) substances in categories 1A or 1B
which are not on the candidate list exceeding 0.1
Technical Data
percentage by mass: no
The products are registered in the GUT-PRODIS
Information System. The GUT-PRODIS system
Constructional data according to EN 1307
ensures compliance with limitations of various
Name Value Unit
chemicals and Volatile Organic Compounds (VOC)-
Modular carpet tiles, 50 cm x
Product Form - emissions and a ban on the use of all substances that
50 cm
are listed as 'Substances of Very High Concern'
Type of
Tufted carpet - (SVHC) under REACH.
manufacture
Polyamide 6 from 100%
Yarn type - Reference service life
recycled material
The service life of textile floor coverings strongly
Total carpet weight 5268 g/m2 depends on the correct installation taking into account
Secondary backing Bitumen heavy backing - the declared use classification and the adherence to
cleaning and maintenance instructions.
A calculation of the reference service life according to
Performance data of the product in accordance with ISO 15686 is not possible.
the declaration of performance with respect to its Alternatively, a reference service life of 10 years can
essential characteristics according to EN 14041: 2018- be assumed, during which the functional and visual
05, Resilient, textile and laminate floor coverings - quality is guaranteed (BNB, Nutzungsdauer von
Essential characteristics. Bauteilen). The technical service life can be
Additional product properties in accordance with EN significantly longer.
1307 can be found on the Product Information System
PRODIS using the PRODIS registration number of the
product (www.pro-dis.info) or on the manufacturer's
technical information section.
Base materials/Ancillary materials
Name Value Unit
Polyamide 6 24.7 %
Polypropylene 0.6 %
Polyester 10.2 %
LCA: Calculation rules
Declared Unit Modules C3, C4 and D are indicated separately for
three end-of-life scenarios:
1 - landfill disposal
Name Value Unit 2 - municipal waste incineration
Declared unit 1 m2 3 - recovery in a cement plant
Grammage 5268 kg/m2
The declared unit refers to 1 m2 produced textile floor A1-A3 Production:
covering. The output of module A5 'Assembly' is 1 m2 Energy supply and production of the basic material,
installed textile floor covering. processing of secondary material, auxiliary material,
The layer thickness of the specific product covered by transport of the material to the manufacturing site,
the EPD can be found on the Product Information emissions, waste water treatment, packaging material
System PRODIS using the PRODIS registration and waste processing up to the landfill disposal of
number of the product (www.pro-dis.info) or on the residual waste (except radioactive waste). Benefits for
manufacturer's technical information section. generated electricity and steam due to the incineration
of production waste are aggregated.
Biogenic carbon that is stored in renewable material
(wood resin, renewable additives, packaging paper) is
System boundary taken into account as well as the associated carbon
dioxide uptake from the air from which this biogenic
Type of EPD: Cradle-to-gate with options carbon comes.
System boundaries of modules A, B, C, D:
A4 Transport:
3 Environmental Product Declaration modulyss – Tufted tiles, 100% recycled polyamide 6 with a maximum total pile weight
of 1300 g/m2 back2back or comfortback backing
Transport of the packed textile floor covering
from factory gate to the place of installation. C2 Transport:
Transport of the carpet waste to a landfill, to the
A5 Installation: municipal waste incineration plant (MWI) or to the
Installation of the textile floor covering, processing of waste collection facility for recycling.
installation waste and packaging waste up to the
landfill disposal of residual waste (except radioactive C3 Waste processing:
waste), the production of the amount of carpet that C3-1: Landfill disposal needs no waste processing.
occurs as installation waste including its transport to C3-2: Impact from waste incineration (plant with R1 >
the place of installation. 0.6), generated electricity and steam are listed in the
Generated electricity and steam due to the incineration result table as exported energy.
of waste are listed in the result table as exported C3-3: Collection of the carpet waste for recovery in the
energy. cement industry, waste processing (granulating),
Biogenic carbon that is stored in renewable materials transport to the cement plant, emissions from the
in installation waste and packaging paper is released incineration.
as carbon dioxide emissions into the air at the end of
life in module A5. C4 Disposal
Preparation of the floor and auxiliary materials C4-1: Impact from landfill disposal,
(adhesives, fixing agents, PET connectors) are beyond C4-2: The carpet waste leaves the system in module
the system boundaries and not taken into account. C3-2,
C4-3: The pre-processed carpet waste leaves the
B1 Use: system in module C3-3.
Indoor emissions during the use stage. After the first
year, no product-related Volatile Organic Compound D Recycling potential:
(VOC) emissions are relevant due to known VOC Calculated benefits result from materials exclusive
decay curves of the product. secondary materials (net materials).
D-A5: Benefits for generated energy due
B2 Maintenance: to incineration of packaging and installation waste
Cleaning of the textile floor covering for a period of 1 (incineration plant with R1 > 0.6),
year: D-1: Benefits for generated energy due to landfill
Vacuum cleaning – electricity supply disposal of carpet waste at the end-of-life,
Wet cleaning – electricity, water consumption, D-2: Benefits for generated energy due to incineration
production of the cleaning agent, waste water of carpet waste at the end-of-life (incineration plant
treatment with R1 > 0.6),
The declared values in this module have to be D-3: Benefits for saved fossil energy and saved
multiplied by the assumed service life of the floor inorganic material due to recovery of the carpet in a
covering in the building in question. cement plant.
B3 - B5: Comparability
The modules are not relevant within the assumed Basically, a comparison or an evaluation of EPD data
reference service life of 10 years. is only possible if all the data sets to be compared
were created according to EN 15804 and the building
B6 - B7: context, respectively the product-specific
No energy and water input are required for the characteristics of performance, are taken into account.
operation of the carpet in the use stage. The modules
do not cause any environmental impact. Background data are taken from the GaBi database,
2022-2. Remaining data gaps are covered by the
C1 De-construction: ecoinvent 3.7 database, 2020.
The floor covering is de-constructed manually and no
additional environmental impact is caused.
LCA: Scenarios and additional technical information
Characteristic product properties Transport to the construction site (A4)
Information on biogenic Carbon Name Value Unit
Litres of fuel (truck, EURO 0-6
0.012 l/100km
mix)
Name Value Unit Transport distance 700 km
Biogenic carbon content in Capacity utilisation (including
0 kg C 55 %
product at factory gate empty runs)
Biogenic carbon content in
accompanying packaging at 0.06 kg C Installation in the building (A5)
factory gate Name Value Unit
1 kg biogenic Carbon is equivalent to 44/12 kg of CO Material loss 0.158 kg
2
Polyethylene packaging waste and installation waste
are considered to be incinerated in a municipal waste
incineration plant. Cardboard packaging waste is going
to be recycled.
Preparation of the floor and auxiliaries (adhesives,
4 Environmental Product Declaration modulyss – Tufted tiles, 100% recycled polyamide 6 with a maximum total pile weight
of 1300 g/m2 back2back or comfortback backing
fixing agents, PET connectors etc.) are not taken into
account. Reuse, recovery and/or recycling potentials (D),
relevant scenario information
Maintenance (B2) Recovery or recycling potentials due to the three end-
The values for cleaning refer to 1 m2 floor covering per of-life scenarios (module C) are indicated separately.
year.
Depending on the application based on ISO 10874, the Recycling in the cement industry (scenario 3)
technical service life recommended by the The organic material of the carpet is used as an
manufacturer and the anticipated strain on the floor by alternative fuel in a cement kiln. It mainly substitutes
customers, the case-specific useful life can be for lignite (68.8 %), hard coal (23.6 %) and petrol coke
established. Based on this useful life the effects of (7.6 %). The inorganic material is substantially
module B2 need to be calculated in order to obtain the integrated into the cement clinker and substitutes for
overall environmental impacts. original material input. VDZ e.V.
Name Value Unit
Maintenance cycle (vacuum Number
208
cleaning) /year
Number
Maintenance cycle (wet cleaning) 1,5
/year
Water consumption (wet cleaning) 0.004 m3
Cleaning agent (wet cleaning) 0.09 kg
Electricity consumption 0.314 kWh
For further information on cleaning and maintenance
see www.modulyss.com
Service life
Name Value Unit
Life Span (according to BBSR) 10 a
Corresponds to
Declared product properties (at the
-
the gate) and finishes specifications of
EN 1307
An assumed quality of work, when Conforms to the
installed in accordance with the manufacturer's -
manufacturer’s instructions instructions
Use in areas
defined by the
Usage conditions, e.g. frequency
use class -
of use, mechanical exposure
according to EN
1307
Maintenance e.g. required According to the
frequency, type and quality and manufacturers -
replacement of components instructions
End of Life (C1-C4)
Three different end-of-life scenarios are declared and
the results are indicated separately in module C.
Each scenario is calculated as a 100 % scenario.
Scenario 1: 100 % landfill disposal
Scenario 2: 100 % municipal waste incineration (MWI)
with R1 > 0.6
Scenario 3: 100 % recovery in the cement industry
If combinations of these scenarios have to be
calculated this should be done according to the
following scheme:
EOL-impact = x % impact (Scenario 1)
+ y % impact (Scenario 2)
+ z % impact (Scenario 3)
with x % + y % + z % = 100 %
Name Value Unit
Collected as mixed construction
5.268 kg
waste (scenarios 1 and 2)
Collected separately (scenario 3) 5.268 kg
Landfilling (scenario 1) 5.268 kg
Energy recovery (scenario 2) 5.268 kg
Energy recovery (scenario 3) 2.810 kg
Recycling (scenario 3) 2.458 kg
5 Environmental Product Declaration modulyss – Tufted tiles, 100% recycled polyamide 6 with a maximum total pile weight
of 1300 g/m2 back2back or comfortback backing
LCA: Results
The LCA results refer to all declared products with a maximum total pile weight of 1300 g/m2. LCA results for
products with a maximum total pile weight of 480 g/m2 can be taken from the corresponding tables of the annexe.
Results for specific products with any other total pile weight can be calculated by using equation 1 given in the
annexe (see annexe chapter: 'General Information on the annexe'). The declared result figures in module B2 have
to be multiplied by the assumed service life (in years) of the floor covering in the building under consideration.
Information on non-relevant modules: Modules B3 - B7 are not relevant during the service life of the carpet.
Modules C1, C3/1, C4/2 and C4/3 cause no additional impact (see chapter "LCA: Calculation rules" in this
document). All these modules are declared and marked as 'modules not relevant/declared'. Module C2 represents
the transport for scenarios 1, 2 and 3. Column D represents module D/A5.
DESCRIPTION OF THE SYSTEM BOUNDARY (X = INCLUDED IN LCA; ND = MODULE OR INDICATOR NOT
DECLARED; MNR = MODULE NOT RELEVANT)
BENEFITS AND
CONSTRUCTI LOADS
PRODUCT STAGE ON PROCESS USE STAGE END OF LIFE STAGE BEYOND THE
STAGE SYSTEM
BOUNDARIES
6 Environmental Product Declaration modulyss – Tufted tiles, 100% recycled polyamide 6 with a maximum total pile weight
of 1300 g/m2 back2back or comfortback backing
lairetam
waR
ylppus tropsnarT
gnirutcafunaM
eht
morf
tropsnarT
etis
eht
ot
etag
ylbmessA esU
ecnanetniaM
riapeR
tnemecalpeR tnemhsibrufeR
ygrene
lanoitarepO esu
retaw
lanoitarepO esu
noitcurtsnoc-eD
noitilomed tropsnarT
gnissecorp
etsaW
lasopsiD -esueR -yrevoceR -gnilcyceR laitnetop
A1 A2 A3 A4 A5 B1 B2 B3 B4 B5 B6 B7 C1 C2 C3 C4 D
X X X X X X X MNR MNR MNR ND ND X X X X X
RESULTS OF THE LCA - ENVIRONMENTAL IMPACT according to EN 15804+A2: 1 m² floor covering
Core Indicator Unit A1-A3 A4 A5 B1 B2 C1 C2 C3/2 C3/3 C4/1 D D/1 D/2 D/3
GWP-total [kg CO2-Eq.] 5.43E+03.21E-1 5.99E-10.00E+04.16E-10.00E+01.79E-26.56E+06.63E+03.70E-1-1.98E-20.00E+0-4.11E-1-2.67E-1
GWP-fossil [kg CO2-Eq.] 5.58E+03.15E-1 3.90E-10.00E+02.15E-10.00E+01.76E-26.56E+06.63E+03.73E-1-1.97E-20.00E+0-4.09E-1-2.66E-1
GWP-biogenic [kg CO2-Eq.] -1.63E-14.08E-3 2.08E-10.00E+04.16E-30.00E+02.27E-4 8.57E-4 1.67E-30.00E+0-9.97E-50.00E+0-2.06E-3-4.60E-4
GWP-luluc [kg CO2-Eq.] 8.91E-3 1.78E-3 3.33E-40.00E+01.96E-10.00E+09.94E-5 2.60E-4 5.14E-4 1.82E-4-2.14E-60.00E+0-4.41E-5-1.29E-4
1.92E- 4.49E- 1.07E- 5.78E- 9.76E- 5.02E- -1.31E- -2.70E- -3.30E-
ODP [kg CFC11-Eq.] 1.50E-8 0.00E+03.42E-80.00E+0 0.00E+0
14 10 15 13 13 13 13 12 13
AP [mol H+-Eq.] 2.12E-2 1.91E-3 8.93E-40.00E+08.32E-40.00E+01.06E-4 6.49E-3 6.81E-3 1.11E-3-2.57E-50.00E+0-5.31E-4-1.03E-3
EP-freshwater [kg P-Eq.] 7.69E-5 9.55E-7 2.37E-60.00E+05.19E-60.00E+05.32E-8 9.55E-7 1.17E-6 6.97E-5-2.67E-80.00E+0-5.50E-7-2.87E-7
EP-marine [kg N-Eq.] 7.34E-3 9.35E-4 3.46E-40.00E+01.97E-40.00E+05.21E-5 3.18E-3 3.32E-3 2.45E-4-6.99E-60.00E+0-1.45E-4-3.09E-4
EP-terrestrial [mol N-Eq.] 6.75E-2 1.04E-2 3.43E-30.00E+02.83E-30.00E+05.77E-4 3.54E-2 3.70E-2 2.69E-3-7.49E-50.00E+0-1.55E-3-3.38E-3
POCP [kg NMVOC-Eq.]1.83E-2 1.77E-3 8.50E-4 4.18E-4 9.83E-40.00E+09.85E-5 8.14E-3 8.42E-3 7.88E-4-1.96E-50.00E+0-4.06E-4-9.21E-4
ADPE [kg Sb-Eq.] 1.90E-6 2.68E-8 5.89E-80.00E+02.30E-70.00E+01.49E-9 3.16E-8 4.27E-8 2.59E-8-2.94E-90.00E+0-6.07E-8-2.57E-8
- -
ADPF [MJ] 1.19E+24.28E+03.82E+00.00E+05.90E+00.00E+02.38E-13.76E+04.85E+05.30E+0-3.34E-10.00E+0
6.95E+03.01E+1
[m³ world-Eq
WDP 7.49E+02.86E-3 2.52E-10.00E+09.99E-20.00E+01.60E-4 8.65E-1 8.71E-1-3.96E-3-2.05E-30.00E+0-4.21E-2-3.83E-2
deprived]
GWP = Global warming potential; ODP = Depletion potential of the stratospheric ozone layer; AP = Acidification potential of land and water; EP =
Caption Eutrophication potential; POCP = Formation potential of tropospheric ozone photochemical oxidants; ADPE = Abiotic depletion potential for non-
fossil resources; ADPF = Abiotic depletion potential for fossil resources; WDP = Water (user) deprivation potential
RESULTS OF THE LCA - INDICATORS TO DESCRIBE RESOURCE USE according to EN 15804+A2: 1 m²
floor covering
Indicator Unit A1-A3 A4 A5 B1 B2 C1 C2 C3/2 C3/3 C4/1 D D/1 D/2 D/3
PERE [MJ] 6.47E+1 2.43E-1 2.23E+0 0.00E+0 3.69E+0 0.00E+0 1.36E-2 6.29E-1 9.34E-1 4.36E-1 -9.07E-2 0.00E+0 -1.87E+0-3.85E-1
PERM [MJ] 2.54E-1 0.00E+0 -2.54E-1 0.00E+0 0.00E+0 0.00E+0 0.00E+0 0.00E+0 0.00E+0 0.00E+0 0.00E+0 0.00E+0 0.00E+0 0.00E+0
PERT [MJ] 6.50E+1 2.43E-1 1.98E+0 0.00E+0 3.69E+0 0.00E+0 1.36E-2 6.29E-1 9.34E-1 4.36E-1 -9.07E-2 0.00E+0 -1.87E+0-3.85E-1
PENRE [MJ] 8.61E+1 4.29E+0 4.04E+0 0.00E+0 5.90E+0 0.00E+0 2.39E-1 3.65E+1 3.76E+1 5.30E+0 -3.34E-1 0.00E+0 -6.95E+0-3.01E+1
PENRM [MJ] 3.29E+1 0.00E+0 -2.15E-1 0.00E+0 0.00E+0 0.00E+0 0.00E+0 -3.27E+1-3.27E+1 0.00E+0 0.00E+0 0.00E+0 0.00E+0 0.00E+0
PENRT [MJ] 1.19E+2 4.29E+0 3.82E+0 0.00E+0 5.90E+0 0.00E+0 2.39E-1 3.77E+0 4.85E+0 5.30E+0 -3.34E-1 0.00E+0 -6.95E+0-3.01E+1
SM [kg] 4.11E+0 0.00E+0 1.23E-1 0.00E+0 0.00E+0 0.00E+0 0.00E+0 0.00E+0 0.00E+0 0.00E+0 0.00E+0 0.00E+0 0.00E+0 1.90E-1
RSF [MJ] 0.00E+0 0.00E+0 0.00E+0 0.00E+0 0.00E+0 0.00E+0 0.00E+0 0.00E+0 0.00E+0 0.00E+0 0.00E+0 0.00E+0 0.00E+0 0.00E+0
NRSF [MJ] 0.00E+0 0.00E+0 0.00E+0 0.00E+0 0.00E+0 0.00E+0 0.00E+0 0.00E+0 0.00E+0 0.00E+0 0.00E+0 0.00E+0 0.00E+0 0.00E+0
FW [m³] 1.79E-1 2.75E-4 6.02E-3 0.00E+0 3.34E-3 0.00E+0 1.53E-5 2.05E-2 2.08E-2 6.20E-5 -8.66E-5 0.00E+0 -1.78E-3 -2.84E-3
PERE = Use of renewable primary energy excluding renewable primary energy resources used as raw materials; PERM = Use of
renewable primary energy resources used as raw materials; PERT = Total use of renewable primary energy resources; PENRE = Use of
non-renewable primary energy excluding non-renewable primary energy resources used as raw materials; PENRM = Use of non-
Caption
renewable primary energy resources used as raw materials; PENRT = Total use of non-renewable primary energy resources; SM = Use
of secondary material; RSF = Use of renewable secondary fuels; NRSF = Use of non-renewable secondary fuels; FW = Use of net fresh
water
RESULTS OF THE LCA – WASTE CATEGORIES AND OUTPUT FLOWS according to EN 15804+A2:
1 m² floor covering
Indicator Unit A1-A3 A4 A5 B1 B2 C1 C2 C3/2 C3/3 C4/1 D D/1 D/2 D/3
HWD [kg] 3.75E-3 2.05E-11 1.13E-4 0.00E+0 4.19E-5 0.00E+0 1.14E-125.65E-106.10E-108.17E-10-4.54E-110.00E+0-9.48E-10-2.26E-10
NHWD [kg] 7.07E-1 6.14E-4 6.00E-2 0.00E+0 7.30E-3 0.00E+0 3.42E-5 1.29E+0 1.29E+0 5.25E+0 -1.68E-4 0.00E+0 -3.47E-3 -1.34E-1
RWD [kg] 2.45E-3 5.28E-6 7.79E-5 0.00E+0 3.76E-4 0.00E+0 2.94E-7 1.36E-4 2.15E-4 6.51E-5 -2.60E-5 0.00E+0 -5.35E-4 -8.50E-5
CRU [kg] 0.00E+0 0.00E+0 0.00E+0 0.00E+0 0.00E+0 0.00E+0 0.00E+0 0.00E+0 0.00E+0 0.00E+0 0.00E+0 0.00E+0 0.00E+0 0.00E+0
MFR [kg] 3.50E-2 0.00E+0 1.31E-1 0.00E+0 0.00E+0 0.00E+0 0.00E+0 0.00E+0 1.41E+0 0.00E+0 0.00E+0 0.00E+0 0.00E+0 0.00E+0
MER [kg] 0.00E+0 0.00E+0 0.00E+0 0.00E+0 0.00E+0 0.00E+0 0.00E+0 0.00E+0 0.00E+0 0.00E+0 0.00E+0 0.00E+0 0.00E+0 0.00E+0
EEE [MJ] 0.00E+0 0.00E+0 2.92E-1 0.00E+0 0.00E+0 0.00E+0 0.00E+0 8.60E+0 0.00E+0 0.00E+0 0.00E+0 0.00E+0 0.00E+0 0.00E+0
EET [MJ] 0.00E+0 0.00E+0 5.38E-1 0.00E+0 0.00E+0 0.00E+0 0.00E+0 1.60E+1 8.59E+1 0.00E+0 0.00E+0 0.00E+0 0.00E+0 0.00E+0
HWD = Hazardous waste disposed; NHWD = Non-hazardous waste disposed; RWD = Radioactive waste disposed; CRU = Components
Caption for re-use; MFR = Materials for recycling; MER = Materials for energy recovery; EEE = Exported electrical energy; EET = Exported
thermal energy
RESULTS OF THE LCA – additional impact categories according to EN 15804+A2-optional:
1 m² floor covering
Indicator Unit A1-A3 A4 A5 B1 B2 C1 C2 C3/2 C3/3 C4/1 D D/1 D/2 D/3
[Disease -2.13E-
PM 1.51E-7 1.10E-8 5.74E-9 0.00E+0 6.84E-8 0.00E+06.13E-10 2.83E-8 3.03E-8 1.06E-8 0.00E+0 0.00E+0 -1.44E-8
Incidence] 10
[kBq U235-
IRP 4.08E-1 7.74E-4 1.29E-2 0.00E+0 6.78E-2 0.00E+0 4.31E-5 2.07E-2 3.41E-2 9.61E-3 -4.40E-3 0.00E+0 0.00E+0 -1.02E-2
Eq.]
ETP-fw [CTUe] 6.76E+1 2.97E+0 2.18E+0 3.60E-3 2.69E+0 0.00E+0 1.65E-1 1.85E+0 2.48E+0 5.18E+0 -7.25E-2 0.00E+0 0.00E+0-5.47E+0
-3.36E- -7.26E-
HTP-c [CTUh] 3.07E-9 6.00E-119.69E-110.00E+06.21E-100.00E+03.34E-129.27E-111.07E-102.33E-10 0.00E+0 0.00E+0
12 11
-1.29E-
HTP-nc [CTUh] 1.18E-7 3.56E-9 3.85E-9 2.60E-11 9.46E-9 0.00E+01.98E-10 6.38E-9 7.10E-9 1.95E-8 0.00E+0 0.00E+0 -4.54E-9
10
SQP [-] ND ND ND ND ND 0.00E+0 ND ND ND ND ND ND ND ND
PM = Potential incidence of disease due to PM emissions; IR = Potential Human exposure efficiency relative to U235; ETP-fw = Potential
Caption comparative Toxic Unit for ecosystems; HTP-c = Potential comparative Toxic Unit for humans (cancerogenic); HTP-nc = Potential
comparative Toxic Unit for humans (not cancerogenic); SQP = Potential soil quality index
No substantiated values can be given for the SQP indicator with the existing database.
The result figures given in module B2 refer to a period of 1 year because a reference service life is not declared.
They have to be multiplied by the assumed service life (in years) of the floor covering in the building under
consideration.
Disclaimer 1 – for the indicator “Potential Human exposure efficiency relative to U235”.
This impact category deals mainly with the eventual impact of low-dose ionizing radiation on human health of the
nuclear fuel cycle. It does not consider effects due to possible nuclear accidents, occupational exposure or
radioactive waste disposal in underground facilities. Potential ionizing radiation from the soil, from radon and from
some construction materials is also not measured by this indicator.
Disclaimer 2 – for the indicators “abiotic depletion potential for non-fossil resources”, “abiotic depletion potential
for fossil resources”, “water (user) deprivation potential, deprivation-weighted water consumption”, “potential
comparative toxic unit for ecosystems”, “potential comparative toxic unit for humans – cancerogenic”, “Potential
comparative toxic unit for humans - not cancerogenic”, “potential soil quality index”.
The results of this environmental impact indicator shall be used with care as the uncertainties on these results are
high or as there is limited experience with the indicator.
References
EN 1307 floor coverings – Environmental product declarations –
DIN EN 1307: 2014+A1:2016+A2:2018-05: Textile Product category rules
floor coverings - Classification
ISO 10874
EN 13501-1 DIN EN ISO 10874: 2012+A1:2021-04: Resilient,
DIN EN 13501-1:2019-05: Fire classification of textile and laminate floor coverings - Classification
construction products and building elements - Part 1:
Classification using data from reaction to fire tests ISO 14025
DIN EN /ISO 14025:2011-10/, Environmental labels
EN 14041 and declarations — Type III environmental
DIN EN 14041: 2018-05 and DIN EN 14041: 2008-05: declarations — Principles and procedures
Resilient, textile and laminate floor coverings -
Essential characteristics
ISO 14040
EN 15804 DIN EN ISO 14040:2006+A1:2020 Environmental
DIN EN 15804:2012+A2:2019 + AC:2021, management - Life cycle assessment - Principles and
Sustainability of construction works — Environmental framework
Product Declarations — Core rules for the product
category of construction products ISO 14044
DIN EN ISO 14044:2006+A1:2018+A2:2020
EN 16810 Environmental management - Life cycle assessment -
DIN EN 16810: 2017-08: Resilient, textile and laminate Requirements and guidelines
7 Environmental Product Declaration modulyss – Tufted tiles, 100% recycled polyamide 6 with a maximum total pile weight
of 1300 g/m2 back2back or comfortback backing
ISO 15686 GaBi database
ISO 15686: Buildings and constructed assets - GaBi Software-System and Database for Life Cycle
Service life planning Engineering, thinkstep AG, Leinfelden-Echterdingen,
ISO 15686-1: 2011-05: Part 1: General principles and 2022-2
framework
ISO 15686-2: 2012-05: Part 2: Service life prediction PCR Part A
procedures Product Category Rules for Building-Related Products
ISO 15686-7: 2017-04: Part 7: Performance and Services Part A: Calculation Rules for the Life
evaluation for feedback of service life data Cycle Assessment and Requirements on the Project
from practice Report according to EN 15804+A2:2019, V1.1, Berlin:
ISO 15686-8: 2008-06: Part 8: Reference service life Institut Bauen und Umwelt e.V. (IBU), January 2021
and service-life estimation
PCR Part B
Regulation (EU) No. 305/2011 Product Category Rules for Building-Related Products
Regulation No. 305/2011 Construction Products and Services
Regulation (CPR) of the European Council and of the Part B: Requirements on the EPD for floor coverings,
European Parliament, April 2011 V1.2, Berlin: Institut Bauen und Umwelt e.V. (IBU),
February 2018
General Instructions for the IBU-EPD Program
General Instructions for the EPD-Program of the PRODIS
Institut Bauen und Umwelt e.V., The Preparation of Product Information System (PRODIS) of the
Environmental Product Declarations - EPDs, version European Carpet Industry, Gemeinschaft
2.0, Institut Bauen und Umwelt e.V., Berlin, January umweltfreundlicher Teppichboden e.V (GUT) and
2021, www.ibu-epd.de European Carpet and Rug Association
(ECRA), http://www.pro-dis.info
BNB, Nutzungsdauer von Bauteilen
Bewertungssystem Nachhaltiges Bauen (BNB), REACH
Nutzungsdauer von Bauteilen, Bundesministerium des Regulation (EC) No 1907/2006 of the European
Inneren, für Bau und Heimat, 24.02.2017 Parliament and of the Council of 18 December 2006
concerning the Registration, Evaluation, Authorisation
ECHA candidate list and Restriction of Chemicals (REACH), June 2017,
Candidate List of substances of very high concern last update: 08.07.2021
(SVHCs) for authorisation, 08.07.2021, European
Chemicals Agency (ECHA), Helsinki, Finland VDZ e.V.
Association of German Cement Works, Ed. Environ-
mental Data of the German Cement Industry 2020
ecoinvent
ecoinvent, Zurich, Switzerland, database version 3.7,
published September 2020
8 Environmental Product Declaration modulyss – Tufted tiles, 100% recycled polyamide 6 with a maximum total pile weight
of 1300 g/m2 back2back or comfortback backing
Publisher
Institut Bauen und Umwelt e.V. Tel +49 (0)30 3087748- 0
Hegelplatz 1 Fax +49 (0)30 3087748- 29
10117 Berlin Mail info@ibu-epd.com
Germany Web www.ibu-epd.com
Programme holder
Institut Bauen und Umwelt e.V. Tel +49 (0)30 - 3087748- 0
Hegelplatz 1 Fax +49 (0)30 – 3087748 - 29
10117 Berlin Mail info@ibu-epd.com
Germany Web www.ibu-epd.com
Author of the Life Cycle
Assessment Tel +49 (0)241 96843 410
Gemeinschaft umweltfreundlicher Fax +49 (0)241 96843 400
Teppichboden (GUT) e.V. Mail mail@gut-ev.de
Schönebergstraße 2 Web www.gut-ev.org
52068 Aachen
Germany
Owner of the Declaration
modulyss Tel +32 (0)52 45 72 11
Zevensterrestraat 21 Fax +32 (0)52 44 90 99
9240 Zele Mail info@modulyss.com
Belgium Web www.modulyss.com
