ENVIRONMENTAL PRODUCT DECLARATION
as per ISO 14025 and EN 15804+A2
Owner of the Declaration Gemeinschaft umweltfreundlicher Teppichboden (GUT) e.V.
Programme holder Institut Bauen und Umwelt e.V. (IBU)
Publisher Institut Bauen und Umwelt e.V. (IBU)
Declaration number EPD-GUT-20220341-CBG1-EN
Issue date 01.02.2023
Valid to 31.01.2028
Tufted wall-to-wall carpet - luxury class LC1
with a pile material made of polyamide 6
maximum surface pile weight 400 g/m2,
maximum total pile weight 650 g/m2,
textile backing with a maximum weight of 250 g/m2
Gemeinschaft umweltfreundlicher
Teppichboden (GUT)
www.ibu-epd.com | https://epd-online.com
Umwelt Produktdeklaration Name des Herstellers – Name des Produkts
General Information
Gemeinschaft umweltfreundlicher Tufted wall-to-wall carpet - luxury
Teppichboden (GUT) e.V. class LC1, with a PA 6 pile material,
max. surface pile weight 400 g/m2,
max. total pile weight 650 g/m2, textile
backing with a max. weight of 250 g/m2
Programme holder Owner of the declaration
IBU – Institut Bauen und Umwelt e.V. Gemeinschaft umweltfreundlicher Teppichboden e.V.
Hegelplatz 1 Schönebergstraße 2
10117 Berlin 51068 Aachen
Germany Germany
Declaration number Declared product / declared unit
EPD-GUT-20220341-CBG1-EN 1 m² tufted wall-to-wall carpet, luxury class LC1, PA 6
pile material with a textile backing.
This declaration is based on the product Scope:
category rules: This sample EPD applies to all products of the member
Floor coverings, 02/2018 companies of the Gemeinschaft umweltfreundlicher
(PCR checked and approved by the SVR) Teppichboden (GUT) e.V. that comply with the product
descriptions and are registered in the GUT/PRODIS
information system. It is only valid in conjunction with a
Issue date
valid GUT/PRODIS license of the product.
01.02.2023
The construction and production data of the registered
products are provided by the member companies of
Valid to
the GUT e.V.. The production sites are located in
31.01.2028 Belgium, Denmark, France, Germany, the Netherlands
and Switzerland.
The owner of the declaration shall be liable for the
underlying information and evidence; the IBU shall not
be liable with respect to manufacturer information, life
cycle assessment data and evidences.
The EPD was created according to the specifications
of EN 15804+A2. In the following, the standard will be
simplified as EN 15804.
Verification
The standard EN 15804 serves as the core PCR
Independent verification of the declaration and data
according to ISO 14025:2011
Dipl. Ing. Hans Peters internally x externally
(chairman of Institut Bauen und Umwelt e.V.)
Dr. Alexander Röder Angela Schindler
(Managing Director Institut Bauen und Umwelt e.V.)) (Independent verifier)
Product
Product description/Product definition Regulation (CPR) applies. The product needs a
The declaration applies to tufted wall-to-wall carpets Declaration of Performance (DoP) taking into
having a pile material of polyamide 6 and a textile consideration EN 14041:2018-05, Resilient, textile and
backing with a maximum weight of 250 g/m2. laminate floor coverings - Essential characteristics, and
The products correspond to luxury class LC1 with a the CE-marking. The DoP of the product can be found
limitation of the maximum surface pile weight of 400 on the manufacturer's technical information section.
g/m² and a maximum total pile weight of 650 g/m2. For the application and use of the product the
Colouring and design of the use layer may be achieved respective national provisions apply.
by aqueous dyeing methods or by using solution-dyed
yarns. Application
For the placing on the market of the specific product in The use class of the specific product as defined in
the European Union/European Free Trade Association EN 1307 can be found in the Product Information
(EU/EFTA) (with the exception of Switzerland) System (PRODIS) using the PRODIS registration
Regulation (EU) No. 305/2011 Construction Product number of the product.
2 Environmental Product Declaration GUT e.V. – Tufted wall-to-wall carpet with PA6 pile material and textile backing, LC1
The base materials refer to the fictitious worst-case
Technical Data product representing all products with the described
The technical data describes a fictitious worst-case characteristics.
product representing all products with the described The specific product covered by the EPD contains
characteristics. substances listed in the ECHA candidate list
(08.07.2021) or other carcinogenic, mutagenic or
Constructional data according to EN 1307 reprotoxic (CMR) substances in categories 1A or 1B
Name Value Unit which are not on the candidate list exceeding 0.1
Product Form wall-to-wall carpet on rolls - percentage by mass: no
Type of The products are registered in the GUT-PRODIS
Tufted carpet -
manufacture Information System. The PRODIS system ensures the
Yarn type Polyamide 6 - compliance with limitations of various chemicals and
Total carpet weight max. 2400 g/m2 Volatile Organic Compound (VOC)-emissions and a
Surface pile weight max. 400 g/m2 ban on the use of all substances that are listed as
Secondary backing Textile backing - 'Substances of Very High Concern' (SVHC) under
REACH.
Performance data of the product in accordance with Reference service life
the declaration of performance with respect to its The service life of textile floor coverings strongly
essential characteristics according to EN 14041: 2018- depends on the correct installation taking into account
05, Resilient, textile and laminate floor coverings - the declared use classification and the adherence to
Essential characteristics. cleaning and maintenance instructions.
Additional product properties in accordance with EN A calculation of the reference service life according to
1307 can be found on the Product Information System ISO 15686 is not possible.
PRODIS using the PRODIS registration number of the Alternatively, a reference service life of 10 years can
product (www.pro-dis.info) or on the manufacturer's be assumed, during which the functional and visual
technical information section. quality is guaranteed (BNB, Nutzungsdauer von
Bauteilen). The technical service life can be
Base materials/Ancillary materials significantly longer.
Name Value Unit
Polyamide 6 27.1 %
Polyester 7.9 %
Polypropylene 7.9 %
Mineral Filler 38.9 %
Aluminiumhydroxide 6.3 %
Polymer dispersion (solid content) 7.8 %
Additives 4.1 %
LCA: Calculation rules
Declared Unit System boundaries of modules A, B, C, D:
Modules C3, C4 and D are indicated separately for
three end-of-life scenarios:
Name Value Unit 1 - landfill disposal
Declared unit 1 m2 2 - municipal waste incineration
Grammage 2.4 kg/m2 3 - recovery in a cement plant
The declared unit refers to 1 m2 produced textile floor
covering. The Output of module A5 'Assembly' is 1 m2 A1-A3 Production:
installed textile floor covering. Energy supply and production of the basic material,
The layer thickness of the specific product covered by processing of secondary material, auxiliary material,
the EPD can be found on the Product Information transport of the material to the manufacturing site,
System PRODIS using the PRODIS registration emissions, waste water treatment, packaging material
number of the product (www.pro-dis.info) or on the and waste processing up to the landfill disposal of
manufacturer's technical information section. residual waste (except radioactive waste). Benefits for
generated electricity and steam due to the incineration
The LCA results refer to the fictitious worst-case of production waste are aggregated.
product, which covers all products of the members of Biogenic carbon that is stored in renewable material
the GUT e.V. that correspond to the product (packaging paper) is taken into account as well as the
descriptions and are registered in the GUT/PRODIS associated carbon dioxide uptake from the air from
information system. which this biogenic carbon comes.
A4 Transport:
System boundary Transport of the packed textile floor covering
from factory gate to the place of installation.
Type of EPD:
Cradle-to-gate with options, module C1-C4, module D,
and additional modules A4, A5, B1, B2.
3 Environmental Product Declaration GUT e.V. – Tufted wall-to-wall carpet with PA6 pile material and textile backing, LC1
A5 Installation: C2 Transport:
Installation of the textile floor covering, processing of Transport of the carpet waste to a landfill, to the
installation waste and packaging waste up to the municipal waste incineration plant (MWI) or to the
landfill disposal of residual waste (except radioactive waste collection facility for recycling.
waste), the production of the amount of carpet that
occurs as installation waste including its transport to C3 Waste processing:
the place of installation. C3-1: Landfill disposal needs no waste processing.
Generated electricity and steam due to the incineration C3-2: Impact from waste incineration (plant with
of waste are listed in the result table as exported R1>0.6), generated electricity and steam are listed in
energy. the result table as exported energy.
Biogenic carbon that is stored in renewable materials C3-3: Collection of the carpet waste for recovery in the
in packaging paper is released as carbon dioxide cement industry, waste processing (granulating),
emissions into the air at the end of life in module A5. transport to the cement plant, emissions from the
Preparation of the floor and auxiliary materials incineration.
(adhesives, fixing agents, PET connectors) are beyond
the system boundaries and not taken into account. C4 Disposal
C4-1: Impact from landfill disposal,
B1 Use: C4-2: The carpet waste leaves the system in
Indoor emissions during the use stage. After the first module C3-2,
year, no product-related Volatile Organic Compound C4-3: The pre-processed carpet waste leaves the
(VOC) emissions are relevant due to known VOC system in module C3-3.
decay curves of the product.
D Recycling potential:
B2 Maintenance: Calculated benefits result from materials exclusive
Cleaning of the textile floor covering for a period of 1 secondary materials (net materials).
year: D-A5: Benefits for generated energy due
Vacuum cleaning – electricity supply to incineration of packaging and installation waste
Wet cleaning – electricity, water consumption, (incineration plant with R1 > 0.6),
production of the cleaning agent, waste water D-1: Benefits for generated energy due to landfill
treatment. disposal of carpet waste at the end of life,
The declared values in this module have to be D-2: Benefits for generated energy due to incineration
multiplied by the assumed service life of the floor of carpet waste at the end-of-life (incineration plant
covering in the building in question. with R1 > 0.6),
D-3: Benefits for saved fossil energy and saved
B3 - B5: inorganic material due to recovery of the carpet in a
The modules are not relevant within the assumed cement plant.
reference service life of 10 years.
Comparability
B6 - B7: Basically, a comparison or an evaluation of EPD data
No energy and water input are required for the is only possible if all the data sets to be compared
operation of the carpet in the use stage. The modules were created according to EN 15804 and the building
are not relevant and not declared. context, respectively the product-specific
characteristics of performance, are taken into account.
C1 De-construction:
The floor covering is de-constructed manually and no Background data are taken from the GaBi database,
additional environmental impact is caused. 2021-2. Remaining data gaps are covered by the
ecoinvent 3.7 database, 2020.
LCA: Scenarios and additional technical information
Characteristic product properties Installation in the building (A5)
Information on biogenic carbon Name Value Unit
Material loss 0.216 kg
Polyethylene packaging waste and installation waste
Name Value Unit are considered to be incinerated in a municipal waste
Biogenic carbon content in incineration plant. Cardboard packaging waste is going
accompanying packaging at factory 0.005 kg C to be recycled.
gate Preparation of the floor and auxiliaries (adhesives,
1 kg biogenic Carbon is equivalent to 44/12 kg of CO fixing agents, PET connectors etc.) are not taken into
2
account.
Maintenance (B2)
Transport to the construction site (A4) The values for cleaning refer to 1 m2 floor covering per
Name Value Unit year.
Litres of fuel (truck, EURO 0-6 Depending on the application based on ISO 10874, the
0.0057 l/100km
mix) technical service life recommended by the
Transport distance 700 km manufacturer and the anticipated strain on the floor by
Capacity utilisation (including customers, the case-specific useful life can be
55 %
empty runs) established. Based on this useful life the effects of
module B2 need to be calculated in order to obtain the
4 Environmental Product Declaration GUT e.V. – Tufted wall-to-wall carpet with PA6 pile material and textile backing, LC1
overall environmental impacts. alternative fuel in a cement kiln. It mainly substitutes
for lignite (68.8 %), hard coal (23.6 %) and petrol coke
(7.6 %). The inorganic material is substantially
Name Value Unit integrated into the cement clinker and substitutes for
Maintenance cycle (vacuum Number the original material input. VDZ e.V.
156
cleaning) /year
Number
Maintenance cycle (wet cleaning) 0.92
/year
Water consumption (wet cleaning) 0.0027 m3
Cleaning agent (wet cleaning) 0.055 kg
Electricity consumption 0.326 kWh
The values result from the calculation of a mixed
scenario for use in object areas and in private areas.
Maintenance cycle vacuum cleaning: 4 times per week
in object areas, 2 times per week in private areas.
Maintenance cycle wet cleaning: 3 times per 2 years in
object areas, 1 time per 3 years in private areas.
Service life
Name Value Unit
Life Span (according to BBSR) 10 a
Corresponds to
Declared product properties (at the
-
the gate) and finishes specifications of
EN 1307
An assumed quality of work, when Conforms to the
installed in accordance with the manufacturer's -
manufacturer’s instructions instructions
Use in areas
defined by the
Usage conditions, e.g. frequency
use class -
of use, mechanical exposure
according to EN
1307
Maintenance e.g. required According to the
frequency, type and quality and manufacturers' -
replacement of components instructions
End of Life (C1-C4)
Three different end-of-life scenarios are declared and
the results are indicated separately in module C.
Each scenario is calculated as a 100 % scenario.
Scenario 1: 100 % landfill disposal
Scenario 2: 100 % municipal waste incineration (MWI)
with R1>0.6
Scenario 3: 100 % recovery in the cement industry
If combinations of these scenarios have to be
calculated this should be done according to the
following scheme:
EOL-impact = x % impact (Scenario 1)
+ y % impact (Scenario 2)
+ z % impact (Scenario 3)
with x % + y % + z % = 100 %
Name Value Unit
Collected as mixed construction
2.4 kg
waste (scenarios 1 and 2)
Collected separately (scenario 3) 2.4 kg
Landfilling (scenario 1) 2.4 kg
Energy recovery (scenario 2) 2.4 kg
Energy recovery (scenario 3) 1.316 kg
Recycling (scenario 3) 1.084 kg
Reuse, recovery and/or recycling potentials (D),
relevant scenario information
Recovery or recycling potentials due to the three end
of life scenarios (module C) are indicated separately.
Recycling in the cement industry (scenario 3)
The organic material of the carpet is used as an
5 Environmental Product Declaration GUT e.V. – Tufted wall-to-wall carpet with PA6 pile material and textile backing, LC1
LCA: Results
The modules C3/1, C4/2 and C4/3 cause no additional impact (see chapter "LCA: Calculation rules").
Module C2 represents the transport for scenarios 1, 2 and 3. The values in column D result from module A5.
DESCRIPTION OF THE SYSTEM BOUNDARY (X = INCLUDED IN LCA; ND = MODULE OR INDICATOR NOT
DECLARED; MNR = MODULE NOT RELEVANT)
BENEFITS AND
CONSTRUCTI LOADS
PRODUCT STAGE ON PROCESS USE STAGE END OF LIFE STAGE BEYOND THE
STAGE SYSTEM
BOUNDARIES
6 Environmental Product Declaration GUT e.V. – Tufted wall-to-wall carpet with PA6 pile material and textile backing, LC1
lairetam
waR
ylppus tropsnarT
gnirutcafunaM
eht
morf
tropsnarT
etis
eht
ot
etag
ylbmessA esU
ecnanetniaM
riapeR
tnemecalpeR tnemhsibrufeR
ygrene
lanoitarepO esu
retaw
lanoitarepO esu
noitcurtsnoc-eD
noitilomed tropsnarT
gnissecorp
etsaW
lasopsiD -esueR -yrevoceR -gnilcyceR laitnetop
A1 A2 A3 A4 A5 B1 B2 B3 B4 B5 B6 B7 C1 C2 C3 C4 D
X X X X X X X MNR MNR MNR ND ND X X X X X
RESULTS OF THE LCA - ENVIRONMENTAL IMPACT according to EN 15804+A2: 1 m² floor covering
Core Indicator Unit A1-A3 A4 A5 B1 B2 C1 C2 C3/2 C3/3 C4/1 D D/1 D/2 D/3
-
GWP-total [kg CO2-Eq.] 1.07E+11.48E-11.54E+00.00E+03.85E-10.00E+08.14E-33.48E+03.52E+01.70E-1-2.20E-10.00E+0 1.23E+0-2.66E-1
-
GWP-fossil [kg CO2-Eq.] 1.07E+11.45E-11.52E+00.00E+02.62E-10.00E+07.99E-33.48E+03.52E+01.70E-1-2.19E-10.00E+0 1.22E+0-2.66E-1
GWP-biogenic [kg CO2-Eq.] 3.36E-2 1.88E-3 2.12E-20.00E+02.99E-30.00E+01.03E-4 3.96E-4 7.66E-4 2.04E-8-1.12E-30.00E+0-6.20E-3-2.58E-4
GWP-luluc [kg CO2-Eq.] 2.81E-3 8.20E-4 3.40E-40.00E+01.20E-10.00E+04.54E-5 1.13E-4 2.29E-4 8.28E-5-2.41E-50.00E+0-1.33E-4-1.28E-4
2.37E- 8.83E- 2.17E- 4.87E- 2.55E- 4.36E- 2.29E- -1.48E- -8.16E- -4.31E-
ODP [kg CFC11-Eq.] 0.00E+02.08E-80.00E+0 0.00E+0
11 15 12 16 13 13 13 12 12 13
AP [mol H+-Eq.] 1.64E-2 8.78E-4 1.86E-30.00E+06.17E-40.00E+04.82E-5 3.09E-3 3.24E-3 5.04E-4-2.87E-40.00E+0-1.59E-3-9.17E-4
EP-freshwater [kg P-Eq.] 2.31E-5 4.40E-7 2.16E-60.00E+03.31E-60.00E+02.42E-8 4.09E-7 5.05E-7 3.17E-5-3.01E-70.00E+0-1.67E-6-3.05E-7
EP-marine [kg N-Eq.] 4.67E-3 4.30E-4 6.02E-40.00E+01.45E-40.00E+02.37E-5 1.52E-3 1.58E-3 1.12E-4-7.82E-50.00E+0-4.34E-4-2.91E-4
EP-terrestrial [mol N-Eq.] 4.51E-2 4.77E-3 6.15E-30.00E+01.98E-30.00E+02.64E-4 1.71E-2 1.78E-2 1.22E-3-8.36E-40.00E+0-4.65E-3-3.19E-3
POCP [kg NMVOC-Eq.]1.52E-2 8.13E-4 1.81E-3 4.18E-4 6.66E-40.00E+04.49E-5 3.89E-3 4.02E-3 3.58E-4-2.18E-40.00E+0-1.22E-3-8.78E-4
6.79E-
ADPE [kg Sb-Eq.] 1.65E-6 1.23E-8 1.51E-70.00E+01.54E-70.00E+0 1.41E-8 1.92E-8 1.18E-8-3.31E-80.00E+0-1.83E-7-2.56E-8
10
- - -
ADPF [MJ] 2.17E+21.97E+01.99E+10.00E+04.50E+00.00E+01.09E-11.70E+02.19E+02.42E+0 0.00E+0
3.72E+0 2.07E+13.56E+1
[m³ world-Eq
WDP 6.17E-1 1.32E-3 1.16E-10.00E+07.22E-20.00E+07.27E-5 4.31E-1 4.34E-1-1.81E-3-2.31E-20.00E+0-1.27E-1-4.00E-2
deprived]
GWP = Global warming potential; ODP = Depletion potential of the stratospheric ozone layer; AP = Acidification potential of land and water; EP =
Caption Eutrophication potential; POCP = Formation potential of tropospheric ozone photochemical oxidants; ADPE = Abiotic depletion potential for non-
fossil resources; ADPF = Abiotic depletion potential for fossil resources; WDP = Water (user) deprivation potential
RESULTS OF THE LCA - INDICATORS TO DESCRIBE RESOURCE USE according to EN 15804+A2: 1 m²
floor covering
Indicator Unit A1-A3 A4 A5 B1 B2 C1 C2 C3/2 C3/3 C4/1 D D/1 D/2 D/3
PERE [MJ] 1.97E+1 1.12E-1 1.84E+0 0.00E+0 2.75E+0 0.00E+0 6.17E-3 2.79E-1 4.18E-1 1.99E-1 -1.02E+0 0.00E+0 -5.65E+0-3.58E-1
PERM [MJ] 2.30E-2 0.00E+0 -2.30E-2 0.00E+0 0.00E+0 0.00E+0 0.00E+0 0.00E+0 0.00E+0 0.00E+0 0.00E+0 0.00E+0 0.00E+0 0.00E+0
PERT [MJ] 1.98E+1 1.12E-1 1.82E+0 0.00E+0 2.75E+0 0.00E+0 6.17E-3 2.79E-1 4.18E-1 1.99E-1 -1.02E+0 0.00E+0 -5.65E+0-3.58E-1
PENRE [MJ] 1.75E+2 1.97E+0 2.31E+1 0.00E+0 4.50E+0 0.00E+0 1.09E-1 4.12E+1 4.17E+1 2.42E+0 -3.72E+0 0.00E+0 -2.07E+1-3.56E+1
PENRM [MJ] 4.27E+1 0.00E+0 -3.18E+0 0.00E+0 0.00E+0 0.00E+0 0.00E+0 -3.95E+1-3.95E+1 0.00E+0 0.00E+0 0.00E+0 0.00E+0 0.00E+0
PENRT [MJ] 2.17E+2 1.97E+0 1.99E+1 0.00E+0 4.50E+0 0.00E+0 1.09E-1 1.70E+0 2.19E+0 2.42E+0 -3.72E+0 0.00E+0 -2.07E+1-3.56E+1
SM [kg] 1.04E-2 0.00E+0 9.36E-4 0.00E+0 0.00E+0 0.00E+0 0.00E+0 0.00E+0 0.00E+0 0.00E+0 0.00E+0 0.00E+0 0.00E+0 6.44E-1
RSF [MJ] 0.00E+0 0.00E+0 0.00E+0 0.00E+0 0.00E+0 0.00E+0 0.00E+0 0.00E+0 0.00E+0 0.00E+0 0.00E+0 0.00E+0 0.00E+0 0.00E+0
NRSF [MJ] 0.00E+0 0.00E+0 0.00E+0 0.00E+0 0.00E+0 0.00E+0 0.00E+0 0.00E+0 0.00E+0 0.00E+0 0.00E+0 0.00E+0 0.00E+0 0.00E+0
FW [m³] 3.58E-2 1.26E-4 4.65E-3 0.00E+0 2.52E-3 0.00E+0 6.98E-6 1.02E-2 1.03E-2 2.83E-5 -9.76E-4 0.00E+0 -5.40E-3 -3.22E-3
PERE = Use of renewable primary energy excluding renewable primary energy resources used as raw materials; PERM = Use of
renewable primary energy resources used as raw materials; PERT = Total use of renewable primary energy resources; PENRE = Use of
non-renewable primary energy excluding non-renewable primary energy resources used as raw materials; PENRM = Use of non-
Caption
renewable primary energy resources used as raw materials; PENRT = Total use of non-renewable primary energy resources; SM = Use
of secondary material; RSF = Use of renewable secondary fuels; NRSF = Use of non-renewable secondary fuels; FW = Use of net fresh
water
RESULTS OF THE LCA – WASTE CATEGORIES AND OUTPUT FLOWS according to EN 15804+A2:
1 m² floor covering
Indicator Unit A1-A3 A4 A5 B1 B2 C1 C2 C3/2 C3/3 C4/1 D D/1 D/2 D/3
HWD [kg] 2.44E-8 9.45E-12 2.23E-9 0.00E+0 2.56E-5 0.00E+0 5.21E-132.59E-102.80E-103.72E-10-5.05E-100.00E+0 -2.82E-9-1.55E-10
NHWD [kg] 2.26E-1 2.83E-4 6.96E-2 0.00E+0 5.14E-3 0.00E+0 1.56E-5 5.37E-1 5.37E-1 2.39E+0 -1.88E-3 0.00E+0 -1.04E-2 -7.23E-2
RWD [kg] 4.47E-3 2.43E-6 4.10E-4 0.00E+0 3.74E-4 0.00E+0 1.34E-7 6.12E-5 9.72E-5 2.97E-5 -2.93E-4 0.00E+0 -1.62E-3 -7.38E-5
CRU [kg] 0.00E+0 0.00E+0 0.00E+0 0.00E+0 0.00E+0 0.00E+0 0.00E+0 0.00E+0 0.00E+0 0.00E+0 0.00E+0 0.00E+0 0.00E+0 0.00E+0
MFR [kg] 1.31E-2 0.00E+0 1.32E-2 0.00E+0 0.00E+0 0.00E+0 0.00E+0 0.00E+0 6.44E-1 0.00E+0 0.00E+0 0.00E+0 0.00E+0 0.00E+0
MER [kg] 0.00E+0 0.00E+0 0.00E+0 0.00E+0 0.00E+0 0.00E+0 0.00E+0 0.00E+0 0.00E+0 0.00E+0 0.00E+0 0.00E+0 0.00E+0 0.00E+0
EEE [MJ] 0.00E+0 0.00E+0 9.84E-1 0.00E+0 0.00E+0 0.00E+0 0.00E+0 5.44E+0 0.00E+0 0.00E+0 0.00E+0 0.00E+0 0.00E+0 0.00E+0
EET [MJ] 0.00E+0 0.00E+0 1.77E+0 0.00E+0 0.00E+0 0.00E+0 0.00E+0 9.93E+0 3.95E+1 0.00E+0 0.00E+0 0.00E+0 0.00E+0 0.00E+0
HWD = Hazardous waste disposed; NHWD = Non-hazardous waste disposed; RWD = Radioactive waste disposed; CRU = Components
Caption
for re-use; MFR = Materials for recycling; MER = Materials for energy recovery; EEE = Exported electrical energy; EET = Exported
thermal energy
RESULTS OF THE LCA – additional impact categories according to EN 15804+A2-optional:
1 m² floor covering
Indicator Unit A1-A3 A4 A5 B1 B2 C1 C2 C3/2 C3/3 C4/1 D D/1 D/2 D/3
[Disease
PM 1.23E-7 5.07E-9 1.28E-8 0.00E+0 4.27E-8 0.00E+02.79E-10 1.27E-8 1.36E-8 4.85E-9 -2.39E-9 0.00E+0 -1.32E-8 -1.91E-8
Incidence]
[kBq U235-
IRP 6.86E-1 3.56E-4 6.29E-2 0.00E+0 6.58E-2 0.00E+0 1.96E-5 9.37E-3 1.55E-2 4.38E-3 -4.96E-2 0.00E+0 -2.74E-1 -7.94E-3
Eq.]
ETP-fw [CTUe] 9.34E+1 1.37E+0 8.62E+0 3.60E-3 2.03E+0 0.00E+0 7.54E-2 8.04E-1 1.09E+0 2.36E+0 -8.17E-1 0.00E+0-4.51E+0-6.23E+0
-3.76E- -2.09E- -6.88E-
HTP-c [CTUh] 3.37E-9 2.76E-113.11E-100.00E+03.90E-100.00E+01.52E-124.19E-114.85E-111.06E-10 0.00E+0
11 10 11
HTP-nc [CTUh] 1.52E-7 1.64E-9 1.41E-8 2.60E-11 6.19E-9 0.00E+09.03E-11 2.54E-9 2.87E-9 8.89E-9 -1.44E-9 0.00E+0 -8.02E-9 -3.99E-9
SQP [-] ND ND ND ND ND ND ND ND ND ND ND ND ND ND
PM = Potential incidence of disease due to PM emissions; IR = Potential Human exposure efficiency relative to U235; ETP-fw = Potential
Caption comparative Toxic Unit for ecosystems; HTP-c = Potential comparative Toxic Unit for humans (cancerogenic); HTP-nc = Potential
comparative Toxic Unit for humans (not cancerogenic); SQP = Potential soil quality index
No substantiated values can be given for the SQP indicator with the existing database.
The result figures given in module B2 refer to a period of 1 year because a reference service life is not declared.
They have to be multiplied by the assumed service life (in years) of the floor covering in the building under
consideration.
Disclaimer 1 – for the indicator “Potential Human exposure efficiency relative to U235”.
This impact category deals mainly with the eventual impact of low dose ionizingradiation on human health of the
nuclear fuel cycle. It does not consider effects due to possible nuclear accidents, occupational exposure nor due
to radioactive waste disposal in undergroundfacilities. Potential ionizing radiation from the soil, from radon and
from some construction materials is also not measured by this indicator.
Disclaimer 2 – for the indicators “abiotic depletion potential for non-fossil resources”, “abiotic depletion potential
for fossil resources”, “water (user) deprivation potential, deprivation-weighted water consumption”, “potential
comparative toxic unit for ecosystems”, “potential comparative toxic unit for humans – cancerogenic”, “Potential
comparative toxic unit for humans - not cancerogenic”, “potential soil quality index”.
The results of this environmental impact indicator shall be used with care as the uncertainties on these results are
high or as there is limited experience with the indicator.
References
EN 1307 ISO 14040
DIN EN 1307: 2014+A1:2016+A2:2018-05: Textile DIN EN ISO 14040:2006+A1:2020 Environmental
floor coverings - Classification management - Life cycle assessment - Principles and
framework
EN 13501-1
DIN EN 13501-1:2019-05: Fire classification of ISO 14044
construction products and building elements - Part 1: DIN EN ISO 14044:2006+A1:2018+A2:2020
Classification using data from reaction to fire tests Environmental management - Life cycle assessment -
Requirements and guidelines
EN 14041
DIN EN 14041: 2018-05 and DIN EN 14041: 2008-05: ISO 15686
Resilient, textile and laminate floor coverings - ISO 15686: Buildings and constructed assets -
Essential characteristics Service life planning
ISO 15686-1: 2011-05: Part 1: General principles and
EN 15804 framework
DIN EN 15804:2012+A2:2019 + AC:2021, ISO 15686-2: 2012-05: Part 2: Service life prediction
Sustainability of construction works — Environmental procedures
Product Declarations — Core rules for the product ISO 15686-7: 2017-04: Part 7: Performance
category of construction products evaluation for feedback of service life data
from practice
EN 16810 ISO 15686-8: 2008-06: Part 8: Reference service life
DIN EN 16810: 2017-08: Resilient, textile and laminate and service-life estimation
floor coverings – Environmental product declarations –
Product category rules Regulation (EU) No. 305/2011
Regulation No. 305/2011 Construction Products
ISO 10874 Regulation (CPR) of the European Council and of the
DIN EN ISO 10874: 2012+A1:2021-04: Resilient, European Parliament, April 2011
textile and laminate floor coverings - Classification
General Instructions for the IBU-EPD Program
ISO 14025 General Instructions for the EPD-Program of the
DIN EN /ISO 14025:2011-10/, Environmental labels Institut Bauen und Umwelt e.V., The Preparation of
and declarations — Type III environmental Environmental Product Declarations - EPDs, version
declarations — Principles and procedures
7 Environmental Product Declaration GUT e.V. – Tufted wall-to-wall carpet with PA6 pile material and textile backing, LC1
2.0, Institut Bauen und Umwelt e.V., Berlin, January PCR Part B
2021, www.ibu-epd.de Product Category Rules for Building-Related Products
and Services
BNB, Nutzungsdauer von Bauteilen Part B: Requirements on the EPD for floor coverings,
Bewertungssystem Nachhaltiges Bauen (BNB), V1.2, Berlin: Institut Bauen und Umwelt e.V. (IBU),
Nutzungsdauer von Bauteilen, Bundesministerium des February 2018
Inneren, für Bau und Heimat, 24.02.2017
PRODIS
ECHA candidate list Product Information System (PRODIS) of the
Candidate List of substances of very high concern European Carpet Industry, Gemeinschaft
(SVHCs) for authorisation, 08.07.2021, European umweltfreundlicher Teppichboden e.V (GUT) and
Chemicals Agency (ECHA), Helsinki, Finland European Carpet and Rug Association
(ECRA), http://www.pro-dis.info
ecoinvent
ecoinvent, Zurich, Switzerland, database version 3.7, REACH
published September 2020 Regulation (EC) No 1907/2006 of the European
Parliament and of the Council of 18 December 2006
GaBi database concerning the Registration, Evaluation, Authorisation
GaBi Software-System and Database for Life Cycle and Restriction of Chemicals (REACH), June 2017,
Engineering, thinkstep AG, Leinfelden-Echterdingen, last update: 08.07.2021
2022-1
VDZ e.V.
PCR Part A Association of German Cement Works, Ed. Environ-
Product Category Rules for Building-Related Products mental Data of the German Cement Industry 2020
and Services Part A: Calculation Rules for the Life
Cycle Assessment and Requirements on the Project
Report according to EN 15804+A2:2019, V1.2, Berlin:
Institut Bauen und Umwelt e.V. (IBU), November 2021
8 Environmental Product Declaration GUT e.V. – Tufted wall-to-wall carpet with PA6 pile material and textile backing, LC1
Publisher
Institut Bauen und Umwelt e.V. Tel +49 (0)30 3087748- 0
Hegelplatz 1 Fax +49 (0)30 3087748- 29
10117 Berlin Mail info@ibu-epd.com
Germany Web www.ibu-epd.com
Programme holder
Institut Bauen und Umwelt e.V. Tel +49 (0)30 - 3087748- 0
Hegelplatz 1 Fax +49 (0)30 – 3087748 - 29
10117 Berlin Mail info@ibu-epd.com
Germany Web www.ibu-epd.com
Author of the Life Cycle
Assessment Tel +49 (0)241 96843 410
Gemeinschaft umweltfreundlicher Fax +49 (0)241 96843 400
Teppichboden (GUT) e.V. Mail mail@gut-ev.de
Schönebergstraße 2 Web www.gut-ev.org
52068 Aachen
Germany
Owner of the Declaration
Gemeinschaft umweltfreundlicher Tel +49 (0)241 96843 410
Teppichboden (GUT) e.V. Fax +49 (0)241 96843 400
Schönebergstraße 2 Mail mail@gut-ev.de
52068 Aachen Web www.gut-ev.org
Germany
