Environmental product declaration
in accordance with ISO 14025 and EN 15804+A2
Glamox heating H40 H 08
Owner of the declaration: Program operator:
Adax AS The Norwegian EPD Foundation
Product: Declaration number:
Glamox heating H40 H 08
NEPD-7945-7609-EN
Declared unit:
1 pcs Registration number:
This declaration is based on Product Category NEPD-7945-7609-EN
Rules:
Issue date: 30.10.2024
CEN Standard EN 15804:2012+A2:2019
The Norwegian EPD Foundation PCR EPD Italy 007 - Electronic and electrical products Valid to: 30.10.2029
and systems - Electrical heaters
EPD software:
LCAno EPD generator ID: 483655
1 / 14
General information
Product Owner of the declaration:
Glamox heating H40 H 08 Adax AS
Contact person: Justinas Kulbe
Phone: +370 61579835
e-mail: justinas.kulbe@adax.no
Program operator: Manufacturer:
The Norwegian EPD Foundation Adax AS
Post Box 5250 Majorstuen, 0303 Oslo, Norway Myhres gate 1
Phone: +47 977 22 020 3060 Svelvik, Norway
web: www.epd-norge.no
Declaration number: Place of production:
Adax production site(UAB ADAX) - Panevezys (Lithuania)
NEPD-7945-7609-EN
Ramygalos g. 190E
36224 Panevezys, Lithuania
This declaration is based on Product Category Rules: Management system:
CEN Standard EN 15804:2012+A2:2019 ISO - 9001, 14001 and 45001
PCR EPD Italy 007 - Electronic and electrical products and systems -
Electrical heaters
Statement of liability: Organisation no:
The owner of the declaration shall be liable for the underlying 991678891
information and evidence. EPD Norway shall not be liable with respect
to manufacturer information, life cycle assessment data and
evidences.​
Declared unit: Issue date:
1 pcs Glamox heating H40 H 08 30.10.2024
Declared unit with option: Valid to:
A1,A2,A3,A4,A5,B6,C1,C2,C3,C4,D 30.10.2029
Year of study:
2023
Functional unit: Comparability:
1 pc of Glamox heating H40 H 08, installed and used to warm an EPD of construction products may not be comparable if they not
indoor environment, during a service life of 17 years, including waste comply with EN 15804 and seen in a building context.
treatment at end-of-life.
General information on verification of EPD from EPD tools: Development and verification of EPD:
Independent verification of data, other environmental information The declaration is created using EPD tool lca.tools ver EPD2022.03,
and the declaration according to ISO 14025:2010, § 8.1.3 and § 8.1.4. developed by LCA.no. The EPD tool is integrated in the company's
Verification of each EPD is made according to EPD-Norway’s management system, and has been approved by EPD Norway.
guidelines for verification and approval requiring that tools are i)
integrated into the company's environmental management system, ii) Developer of EPD: Zohaib Ali
the procedures for use of the EPD tool are approved by EPD-Norway,
Reviewer of company-specific input data and EPD:​ Børge Heggen
and iii) the process is reviewed annually by an independent third
Johansen, Energiråd AS
party verifier. See Appendix G of EPD-Norway's General Programme
Instructions for further information on EPD tools
Verification of EPD tool: Approved:
Independent third party verification of the EPD tool, background data
and test-EPD in accordance with EPDNorway's procedures and
guidelines for verification and approval of EPD tools. Approval
number: NEPDT78.
Third party verifier:
Elisabet Amat, GREENIZE projects
(no signature required)
2 / 14
Product
Product description:
Glamox Heating H40 is a steel front panel heater with a contemporary Nordic design
Product specification
Choose from several different thermostats: WIFI (WT2), Digital (DT), and slave modules: SLX, SLA-5/24 and EIB.
Glamox Heating Wifi App
Connect easily to your Wi-Fi router at home, at the office or at your cabin.
H40 is splashproof IP24, double insulated Cl. II and has overheating protection.
5 years warranty
Available as high (H:330mm) and low (L:210mm)
Available in 230V and 400V
Available in three colors: White RAL 9016, Sparkling Grey and Pearl Black RAL 7021.
Can be mounted on floor stand (optional).
Materials kg %
Chemical 0,10 2,17
Electronic - Cable 0,12 2,60
Electronic - LED chip 0,00 0,07
Electronic - Wire 0,02 0,46
Electronic component 0,43 9,42
Metal - Alloy 0,01 0,17
Plastic 0,31 6,73
Printed paper 0,00 0,02
Metal - Aluminium 0,06 1,33
Metal - Steel 3,55 77,04
Total 4,60 100,00
Packaging kg %
Packaging - Cardboard 0,50 88,29
Packaging - Paper 0,06 10,17
Packaging - Plastic 0,01 1,55
Total incl. packaging 5,17 100,00
Technical data:
Market:
Europe.
Reference service life, product
17 years. Standard lifetime for electrical heaters applications, provided in PEP Ecopassport PSR for direct, visible, fixed electric heating appliances.
Reference service life, building or construction works
60 years. Standard service life for buildings according to the PCR Part A of EPD Norway.
LCA: Calculation rules
Declared unit:
1 pcs Glamox heating H40 H 08
Cut-off criteria:
All major raw materials and all the essential energy is included. The production processes for raw materials and energy flows with very small
amounts (less than 1%) are not included. These cut-off criteria do not​ apply for hazardous materials and substances.
Allocation:
The allocation is made in accordance with the provisions of EN 15804. Incoming energy and water and waste production in-house is allocated
equally among all products through mass allocation. Effects of primary production of recycled materials is allocated to the main product in which
the material was used. The recycling process and transportation of the material is allocated to this analysis.
Data quality:
Specific data for the product composition are provided by the manufacturer. The data represent the production of the declared product and were
collected for EPD development in the year of study. Background data is based on EPDs according to EN 15804 and different LCA databases. The
data quality of the raw materials in A1 is presented in the table below.
3 / 14
Materials Source Data quality Year
Chemical Ecoinvent 3.6 Database 2019
Electronic - Cable ecoinvent 3.6 Database 2019
Scientific
Electronic - LED chip Scholand et al. (2012) + Ecoinvent 3.6 literature + 2017
database
Supplier data +
Electronic - Wire Product composition + ecoinvent 3.6 2019
database
Electronic component ecoinvent 3.6 Database 2019
Supplier data +
Electronic component Product composition + ecoinvent 3.6 2019
database
Metal - Alloy Ecoinvent 3.6 Database 2019
Metal - Aluminium ecoinvent 3.6 Database 2019
Metal - Steel ecoinvent 3.6 Database 2019
Packaging - Cardboard ecoinvent 3.6 Database 2019
Packaging - Paper ecoinvent 3.6 Database 2019
Packaging - Plastic Ecoinvent 3.6 Database 2019
Plastic ecoinvent 3.6 Database 2019
Plastic Modified ecoinvent 3.6 Database 2019
Printed paper Ecoinvent 3.6 Database 2019
4 / 14
System boundaries (X=included, MND=module not declared, MNR=module not relevant)
Construction Beyond the system
Product stage Use stage End of life stage
installation stage boundaries
A1 A2 A3 A4 A5 B1 B2 B3 B4 B5 B6 B7 C1 C2 C3 C4 D
X X X X X MND MND MND MND MND X MND X X X X X
System boundary:
Additional technical information:
The reference product have different configurations but have the same main functionality, product standards and manufacturing technology, so
extrapolation rules are established according to PEP Ecopassport PSR-0002-ed3.0 -EN-2023 06 06. The main differences in the product family
include :
- Power (W)
- Weight (kg)
The different life cycle modules can be extrapolated to other mentioned configurations of the same product by applying a rule of proportionality to
the parameters, presented in the table "Additional Technical Data". To calculate the environmental impacts for each different variant, the results of
the reference product "Glamox heating H40 H 08" must be multiplied by the factor from the table ""Additional Technical Data".
waR slairetam tropsnarT gnirutcafunaM tropsnarT ylbmessA e​sU ecnanetniaM riapeR tnemecalpeR tnemhsibrufeR lanoitarepO ygrene esu lanoitarepO esu retaw -eD noitcurtsnoc noitilomed tropsnarT etsaW gnissecorp lasopsiD -yrevoceR-esueR laitnetop-gnilcyceR
5 / 14
Product Name Weight (kg) Power (W) Extrapolation factor "All other " phases Extrapolation factor "Use" phase
Glamox Heating H40 H 02 3.85 250 0.75 0.31
Glamox Heating H40 H 04 4.15 400 0.80 0.5
Glamox Heating H40 H 06 4.65 600 0.90 0.75
Glamox Heating H40 H 08 5.17 800 1.00 1.00
Glamox Heating H40 H 10 5.55 1000 1.07 1.25
Glamox Heating H40 H 12 6.45 1200 1.25 1.50
Glamox Heating H40 H 14 7.15 1400 1.38 1.75
Glamox Heating H40 H 20 8.95 2000 1.73 2.50
Glamox Heating H40 L 02 3.24 250 0.63 0.31
Glamox Heating H40 L 04 3.74 400 0.72 0.50
Glamox Heating H40 L 06 4.54 600 0.88 0.75
Glamox Heating H40 L 08 5.24 800 1.01 1.00
Glamox Heating H40 L 10 6.04 1000 1.17 1.25
Glamox Heating H40 L 12 6.64 1200 1.29 1.50
Glamox Heating H40 L 14 7.84 1400 1.52 1.75
Adax Neo H 02 3.85 250 0.75 0.31
Adax Neo H 04 4.15 400 0.8 0.50
Adax Neo H 06 4.65 600 0.90 0.75
Adax Neo H 08 5.17 800 1.00 1.00
Adax Neo H 10 5.55 1000 1.07 1.25
Adax Neo H 12 6.45 1200 1.25 1.50
Adax Neo H 14 7.15 1400 1.38 1.75
Adax Neo H 20 8.95 2000 1.73 2.50
Adax Neo L 02 3.24 250 0.63 0.31
Adax Neo L 04 3.74 400 0.72 0.50
Adax Neo L 06 4.54 600 0.88 0.75
Adax Neo L 08 5.24 800 1.01 1.00
Adax Neo L 10 6.04 1000 1.17 1.25
Adax Neo L 12 6.64 1200 1.29 1.50
Adax Neo L 14 7.84 1400 1.52 1.75
Adax Famn FH 02 3.85 250 0.75 0.31
Adax Famn FH 04 4.15 400 0.80 0.50
Adax Famn FH 06 4.65 600 0.90 0.75
Adax Famn FH 08 5.17 800 1.00 1.00
Adax Famn FH 10 5.55 1000 1.07 1.25
Adax Famn FH 12 6.45 1200 1.25 1.50
Adax Famn FH 14 7.15 1400 1.38 1.75
Adax Famn FH 20 8.95 2000 1.73 2.50
Adax Famn FL 02 3.24 250 0.63 0.31
Adax Famn FL 04 3.74 400 0.72 0.50
Adax Famn FL 06 4.54 600 0.88 0.75
Adax Famn FL 08 5.24 800 1.01 1.00
Adax Famn FL 10 6.04 1000 1.17 1.25
Adax Famn FL 12 6.64 1200 1.29 1.50
Adax Famn FL 14 7.84 1400 1.52 1.75
6 / 14
LCA: Scenarios and additional technical information
The following information describe the scenarios in the different modules of the EPD.
Module A4 = Average distribution into the Europe market (1000 km).
Modules A5 = Installation is performed by manual labor, with the use of electrical machines, that fall under the cut-off criteria of 1% and is
therefore neglected. Packaging of the final product consist of a corrugated board box.
Module B6 :The operational energy use of the electrical heater is calculated based on the methodology provided in PEP Ecopassport PSR-0002-
ed3.0 -EN-2023 06 06. To calculate the electricity use of the electrical heater , the following scenario parameters have been applied:
C = RLT * n * (1-(A + 0.5 * B))
Where:
C: final energy consumption to heat for 17 years, expressed in kWh (17 years is the standard reference lifetime suggested in the PSR).
RLT: number of annual periods defined by the reference lifetime of the reference product, expressed in years.
n = 8760 * P * R * 0.14: 1-year consumption by a direct, visible, fixed electric heating appliance as described in table 6 of the PSR.
8760: hours per year.
P: Thermal power of the reference product in kW.
R: 100 % yield rate of the reference product in %.
14 %: average annual working rate in %.
A: Bonus related to type "A" energy saving functions not requiring a predetermined action by the consumer, as described in table 7 of the PSR and
expressed in %.
B: Bonus related to type "B" energy saving functions requiring a predetermined action by the consumer, as described in table 7 of the PSR and
expressed in %.
Module C1 = The de-installation of the electrical heater is carried out manually, with the assistance of electrical tools. The energy consumption of
portable electrical devices (e.g., drills) is typically low, falling below the 1% cut-off criterion, and is therefore disregarded.
Module C2 = Transportation from building site to the waste treatment facility with an average distance of 300km.
Modules C3 and C4 = Waste treatment of the product follows the default values provided in EN 50693, Product Category Rules for life cycle
assessments of electronic and electrical products and systems, table G.4. This table specified how different types of raw materials used in A1 will
likely be treated during the end-of-life of the product. Waste treatments in C3 include material recycling and incineration with and without energy
recovery and fly ash extraction. Disposal in C4 consist of landfilling of different waste fractions and of ashes.
Module D = The recyclability of metals, plastics, and electronic components allows the producers a credit for the net scrap that is produced at the
end of a product’s life. The benefits from recycling of net scrap are described in formula from EN 15804:2012+A2:2019. Substitution of heat and
electricity generated by the incineration with energy recovery of plastic insulation and other parts is also calculated in module D.
Capacity utilisation Value
Transport from production place to user (A4) Distance (km) Fuel/Energy Consumption Unit
(incl. return) % (Liter/tonne)
Truck, 16-32 tonnes, EURO 6 (km) - Europe 36,7 % 1000 0,043 l/tkm 43,00
Assembly (A5) Unit Value
Waste, packaging, label, paper printed,
supercalendered with silicone and adhesive, to kg 0,00
average treatment (kg)
Waste, packaging, plastic parts, polycarbonate,
kg 0,01
PC, to average treatment (kg)
Waste, packaging, plastic film (PET), to average
kg 0,00
treatment (kg)
Waste, packaging, label, paper printed,
supercalendering, with PVC and adhesive to kg 0,00
average treatment (kg)
Waste, packaging, paper printed, to average
kg 0,05
treatment - A5 including transport (kg)
Waste, packaging, kraft paper, unbleached, to
kg 0,01
average treatment - A5 including transport (kg)
Waste, packaging, corrugated board box, to
kg 0,50
average treatment - A5 including transport (kg)
Operational energy (B6) Unit Value
Electricity, European average (kWh) kWh/DU 13760,21
Capacity utilisation Value
Transport to waste processing (C2) Distance (km) Fuel/Energy Consumption Unit
(incl. return) % (Liter/tonne)
Truck, 16-32 tonnes, EURO 6 (km) - Europe 36,7 % 300 0,043 l/tkm 12,90
7 / 14
Waste processing (C3) Unit Value
Copper to recycling (kg) kg 0,03
Waste treatment per kg electronics scrap from
PWB, with components, recycling of metals C3 kg 0,03
(kg)
Waste treatment per kg used PWB, shredding and
kg 0,07
separation - C3 (kg)
Waste treatment of plastic mixture, incineration
kg 0,20
with energy recovery and fly ash extraction (kg)
Waste treatment per kg used electronic plug
kg 0,00
connector, manual seperation (kg)
Waste treatment of hazardous waste, incineration
kg 0,00
with energy recovery and fly ash extraction (kg)
Waste treatment per kg used electronic cable,
kg 0,14
manual seperation (kg)
Steel to recycling (kg) kg 2,84
Waste treatment per kg electronics scrap from
PWB, with components, recycling of metals C3 kg 0,00
(kg)
Waste treatment per kg used PWB, shredding and
kg 0,00
separation - C3 (kg)
Waste treatment of hazardous waste, incineration
kg 0,10
with fly ash extraction (kg)
Aluminium to recycling (kg) kg 0,04
Disposal (C4) Unit Value
Landfilling of steel (kg) kg 0,71
Landfilling of ashes from incineration of Plastic
kg 0,01
mixture, process per kg ashes and residues (kg)
Landfilling of aluminium (kg) kg 0,13
Landfilling of municipal solid waste (kg) kg 0,00
Landfilling of plastic mixture (kg) kg 0,20
Landfilling of mixed metals (kg) kg 0,01
Landfilling of copper (kg) kg 0,02
Landfilling of hazardous waste (kg) kg 0,00
Landfilling of hazardous waste (kg) kg 0,03
Landfilling of ashes from incineration of
Hazardous waste, process per kg ashes and kg 0,02
residues - C4 (kg)
Aluminium to recycling (kg) kg 0,26
Benefits and loads beyond the system
Unit Value
boundaries (D)
Substitution of primary aluminium with net scrap
kg 0,25
(kg)
Substitution of electricity, in Norway (MJ) MJ 0,31
Substitution of primary steel with net scrap (kg) kg 1,89
Substitution of primary copper with net scrap (kg) kg 0,01
Substitution of primary metals with net scrap
kg 0,00
from PWB, with components (kg)
Substitution of primary metals with net scrap
kg 0,01
from PWB, with components (kg)
Substitution of thermal energy, district heating, in
MJ 4,69
Norway (MJ)
8 / 14
LCA: Results
The LCA results are presented below for the declared unit defined on page 2 of the EPD document.
Environmental impact
Indicator Unit A1 A2 A3 A4 A5
GWP-total kg CO2 -eq 3,91E+01 1,07E+00 1,77E+00 8,45E-01 9,52E-01
GWP-fossil kg CO2 -eq 3,96E+01 1,07E+00 1,73E+00 8,44E-01 1,05E-02
GWP-biogenic kg CO2 -eq -5,76E-01 4,42E-04 1,84E-02 3,49E-04 9,42E-01
GWP-luluc kg CO2 -eq 6,84E-02 3,80E-04 1,84E-02 3,00E-04 3,03E-06
ODP kg CFC11 -eq 2,72E-06 2,42E-07 2,64E-07 1,91E-07 1,94E-09
AP mol H+ -eq 3,56E-01 3,08E-03 1,00E-02 2,43E-03 4,38E-05
EP-FreshWater kg P -eq 3,90E-03 8,53E-06 5,28E-05 6,74E-06 7,89E-08
EP-Marine kg N -eq 4,64E-02 6,12E-04 1,60E-03 4,80E-04 1,58E-05
EP-Terrestial mol N -eq 8,24E-01 6,84E-03 1,94E-02 5,37E-03 1,57E-04
POCP kg NMVOC -eq 1,55E-01 2,61E-03 5,28E-03 2,06E-03 4,54E-05
ADP-minerals&metals1 kg Sb-eq 1,83E-02 2,95E-05 1,20E-05 2,33E-05 2,22E-07
ADP-fossil1 MJ 4,79E+02 1,62E+01 3,15E+01 1,28E+01 1,29E-01
WDP1 m3 2,20E+03 1,56E+01 2,51E+03 1,23E+01 1,75E-01
Indicator Unit B6 C1 C2 C3 C4 D
GWP-total kg CO2 -eq 5,89E+03 0,00E+00 2,53E-01 7,38E-01 5,18E-02 -4,99E+00
GWP-fossil kg CO2 -eq 5,84E+03 0,00E+00 2,53E-01 7,37E-01 5,11E-02 -4,93E+00
GWP-biogenic kg CO2 -eq 4,10E+01 0,00E+00 1,05E-04 6,37E-04 6,18E-04 -1,32E-02
GWP-luluc kg CO2 -eq 1,36E+01 0,00E+00 9,01E-05 1,35E-04 7,12E-05 -4,51E-02
ODP kg CFC11 -eq 4,94E-04 0,00E+00 5,73E-08 2,87E-08 4,87E-09 -1,98E-03
AP mol H+ -eq 3,41E+01 0,00E+00 7,28E-04 5,79E-04 1,63E-04 -6,55E-02
EP-FreshWater kg P -eq 6,23E-01 0,00E+00 2,02E-06 6,61E-06 6,59E-07 -4,40E-04
EP-Marine kg N -eq 4,32E+00 0,00E+00 1,44E-04 1,44E-04 7,63E-05 -6,11E-03
EP-Terrestial mol N -eq 5,33E+01 0,00E+00 1,61E-03 1,57E-03 5,76E-04 -7,13E-02
POCP kg NMVOC -eq 1,35E+01 0,00E+00 6,17E-04 4,22E-04 1,83E-04 -2,56E-02
ADP-minerals&metals1 kg Sb-eq 4,28E-02 0,00E+00 6,99E-06 1,10E-06 1,66E-07 -9,15E-04
ADP-fossil1 MJ 1,20E+05 0,00E+00 3,83E+00 1,37E+00 4,53E-01 -5,40E+01
WDP1 m3 1,81E+06 0,00E+00 3,70E+00 7,41E+00 8,86E+00 -1,19E+03
GWP-total = Global Warming Potential total; GWP-fossil = Global Warming Potential fossil fuels; GWP-biogenic = Global Warming Potential biogenic; GWP-luluc =
Global Warming Potential land use and land use change; ODP = Depletion potential of the stratospheric ozone layer; AP = Acidification potential, Accumulated
Exceedance; EP-freshwater = Eutrophication potential, fraction of nutrients reaching freshwater end compartment: EP-marine = Eutrophication potential, fraction of
nutrients reaching marine end compartment; EP-terrestrial = Eutrophication potential, Accumulated Exceedance; POCP = Formation potential of tropospheric ozone;
ADP-minerals&metals = Abiotic depletion potential for non-fossil resources; ADP-fossil = Abiotic depletion for fossil resources potential; WDP = Water (user)
deprivation potential, deprivation-weighted water consumption
"Reading example: 9,0 E-03 = 9,0*10-3 = 0,009"
*INA Indicator Not Assessed
1. The results of this environmental impact indicator shall be used with care as the uncertainties on these results are high or as there is limited experienced with the
indicator
Remarks to environmental impacts
9 / 14
Additional environmental impact indicators
Indicator Unit A1 A2 A3 A4 A5
PM Disease incidence 3,13E-06 6,54E-08 8,37E-08 5,17E-08 6,46E-10
IRP2 kgBq U235 -eq 1,56E+00 7,07E-02 3,54E-01 5,58E-02 5,52E-04
ETP-fw1 CTUe 2,44E+03 1,20E+01 2,46E+01 9,46E+00 1,75E-01
HTP-c1 CTUh 1,12E-07 0,00E+00 1,37E-09 0,00E+00 5,00E-12
HTP-nc1 CTUh 1,87E-06 1,31E-08 1,91E-08 1,03E-08 2,20E-10
SQP1 dimensionless 1,89E+02 1,13E+01 2,77E+01 8,93E+00 8,99E-02
Indicator Unit B6 C1 C2 C3 C4 D
PM Disease incidence 8,93E-05 0,00E+00 1,55E-08 6,47E-09 2,72E-09 -4,21E-07
IRP2 kgBq U235 -eq 1,05E+03 0,00E+00 1,67E-02 6,28E-03 2,48E-03 -1,46E-01
ETP-fw1 CTUe 8,43E+04 0,00E+00 2,84E+00 6,18E+00 5,36E+02 -4,42E+02
HTP-c1 CTUh 2,35E-06 0,00E+00 0,00E+00 8,19E-10 6,00E-11 -1,74E-08
HTP-nc1 CTUh 8,12E-05 0,00E+00 3,10E-09 3,68E-08 9,14E-10 2,76E-08
SQP1 dimensionless 2,91E+04 0,00E+00 2,68E+00 4,69E-01 9,88E-01 -1,00E+01
PM = Particulate Matter emissions; IRP = Ionizing radiation – human health; ETP-fw = Eco toxicity – freshwater; HTP-c = Human toxicity – cancer effects; HTP-nc =
Human toxicity – non cancer effects; SQP = Potential Soil Quality Index (dimensionless)
"Reading example: 9,0 E-03 = 9,0*10-3 = 0,009"
*INA Indicator Not Assessed
1. The results of this environmental impact indicator shall be used with care as the uncertainties on these results are high or as there is limited experienced with the
indicator
2. This impact category deals mainly with the eventual impact of low dose ionizing radiation on human health of the nuclear fuel cycle. It does not consider effects due
to possible nuclear accidents, occupational exposure nor due to radioactive waste disposal in underground facilities. Potential ionizing radiation from the soil, from
radon and from some construction materials is also not measured by this indicator.
10 / 14
Resource use
Indicator Unit A1 A2 A3 A4 A5
PERE MJ 5,20E+01 2,31E-01 1,52E+01 1,83E-01 2,17E-03
PERM MJ 4,88E+00 0,00E+00 0,00E+00 0,00E+00 -4,87E+00
PERT MJ 5,69E+01 2,31E-01 1,52E+01 1,83E-01 -4,87E+00
PENRE MJ 4,76E+02 1,62E+01 3,16E+01 1,28E+01 1,29E-01
PENRM MJ 1,10E+01 0,00E+00 0,00E+00 0,00E+00 -2,45E-01
PENRT MJ 4,87E+02 1,62E+01 3,16E+01 1,28E+01 -1,16E-01
SM kg 1,95E+00 0,00E+00 0,00E+00 0,00E+00 0,00E+00
RSF MJ 1,32E+00 8,27E-03 5,85E-01 6,53E-03 7,13E-05
NRSF MJ 1,50E-01 2,96E-02 8,01E-02 2,34E-02 2,90E-04
FW m3 3,59E-01 1,73E-03 2,15E-02 1,36E-03 6,26E-05
Indicator Unit B6 C1 C2 C3 C4 D
PERE MJ 2,33E+04 0,00E+00 5,48E-02 2,21E-01 7,55E-02 -1,49E+01
PERM MJ 0,00E+00 0,00E+00 0,00E+00 0,00E+00 0,00E+00 0,00E+00
PERT MJ 2,33E+04 0,00E+00 5,48E-02 2,21E-01 7,55E-02 -1,49E+01
PENRE MJ 1,21E+05 0,00E+00 3,83E+00 1,37E+00 4,53E-01 -5,40E+01
PENRM MJ 0,00E+00 0,00E+00 0,00E+00 -1,07E+01 0,00E+00 0,00E+00
PENRT MJ 1,21E+05 0,00E+00 3,83E+00 -9,34E+00 4,53E-01 -5,40E+01
SM kg 0,00E+00 0,00E+00 0,00E+00 0,00E+00 7,47E-04 6,45E-03
RSF MJ 1,70E+03 0,00E+00 1,96E-03 4,64E-03 1,02E-03 7,13E-02
NRSF MJ 4,04E+02 0,00E+00 7,01E-03 -3,47E-05 7,41E-03 2,07E+00
FW m3 1,02E+02 0,00E+00 4,09E-04 1,66E-03 5,46E-04 -6,93E-02
PERE = Use of renewable primary energy excluding renewable primary energy resources used as raw materials; PERM = Use of renewable primary energy resources used
as raw materials; PERT = Total use of renewable primary energy resources; PENRE = Use of non renewable primary energy excluding non-renewable primary energy
resources used as raw materials; PENRM = Use of non renewable primary energy resources used as raw materials; PENRT = Total use of non renewable primary energy
resources; SM = Use of secondary materials; RSF = Use of renewable secondary fuels; NRSF = Use of non-renewable secondary fuels; FW = Net use of fresh water
"Reading example: 9,0 E-03 = 9,0*10-3 = 0,009"
*INA Indicator Not Assessed
11 / 14
End of life - Waste
Indicator Unit A1 A2 A3 A4 A5
HWD kg 2,50E-01 8,33E-04 3,73E-02 6,58E-04 0,00E+00
NHWD kg 7,80E+00 7,85E-01 1,25E+00 6,21E-01 5,63E-01
RWD kg 1,38E-03 1,10E-04 1,98E-04 8,69E-05 0,00E+00
Indicator Unit B6 C1 C2 C3 C4 D
HWD kg 1,81E+01 0,00E+00 1,97E-04 1,71E-05 6,72E-02 -3,72E-03
NHWD kg 4,08E+02 0,00E+00 1,86E-01 1,23E-01 1,10E+00 -1,61E+00
RWD kg 8,61E-01 0,00E+00 2,61E-05 8,51E-07 2,31E-06 -1,36E-04
HWD = Hazardous waste disposed; NHWD = Non-hazardous waste disposed; RWD = Radioactive waste disposed
"Reading example: 9,0 E-03 = 9,0*10-3 = 0,009"
*INA Indicator Not Assessed
End of life - Output flow
Indicator Unit A1 A2 A3 A4 A5
CRU kg 0,00E+00 0,00E+00 0,00E+00 0,00E+00 0,00E+00
MFR kg 0,00E+00 0,00E+00 1,14E+00 0,00E+00 5,18E-01
MER kg 0,00E+00 0,00E+00 1,95E-02 0,00E+00 4,02E-02
EEE MJ 0,00E+00 0,00E+00 6,81E-03 0,00E+00 3,25E-02
EET MJ 0,00E+00 0,00E+00 1,03E-01 0,00E+00 4,92E-01
Indicator Unit B6 C1 C2 C3 C4 D
CRU kg 0,00E+00 0,00E+00 0,00E+00 0,00E+00 0,00E+00 0,00E+00
MFR kg 0,00E+00 0,00E+00 0,00E+00 2,91E+00 2,58E-01 -2,53E-04
MER kg 0,00E+00 0,00E+00 0,00E+00 3,02E-01 4,43E-07 -3,33E-05
EEE MJ 0,00E+00 0,00E+00 0,00E+00 3,10E-01 2,87E-05 -8,15E-05
EET MJ 0,00E+00 0,00E+00 0,00E+00 4,69E+00 4,34E-04 -1,23E-03
CRU = Components for re-use; MFR = Materials for recycling; MER = Materials for energy recovery; EEE = Exported energy electrical; EET = Exported energy thermal
"Reading example: 9,0 E-03 = 9,0*10-3 = 0,009"
*INA Indicator Not Assessed
Biogenic Carbon Content
Indicator Unit At the factory gate
Biogenic carbon content in product kg C 2,59E-04
Biogenic carbon content in accompanying packaging kg C 2,57E-01
Note: 1 kg biogenic carbon is equivalent to 44/12 kg CO2
12 / 14
Additional requirements
Greenhouse gas emissions from the use of electricity in the manufacturing phase
National production mix from import, low voltage (production of transmission lines, in addition to direct emissions and losses in grid) of applied
electricity for the manufacturing process (A3).
Electricity mix Source Amount Unit
Electricity, Lithuania (kWh) ecoinvent 3.6 373,46 g CO2-eq/kWh
Dangerous substances
The product contains no substances given by the REACH Candidate list.
Indoor environment
Additional Environmental Information
Additional environmental impact indicators required in NPCR Part A for construction products
Indicator Unit A1 A2 A3 A4 A5
GWPIOBC kg CO2 -eq 4,00E+01 1,07E+00 2,28E+00 8,45E-01 1,05E-02
Indicator Unit B6 C1 C2 C3 C4 D
GWPIOBC kg CO2 -eq 6,32E+03 0,00E+00 2,53E-01 7,38E-01 5,49E-02 -5,91E+00
GWP-IOBC: Global warming potential calculated according to the principle of instantaneous oxidation. In order to increase the transparency of biogenic carbon​
contribution to climate impact, the indicator GWP-IOBC is required as it declares climate impacts calculated according to the principle of instantaneous oxidation.​
GWP-IOBC is also referred to as GWP-GHG in context to Swedish public procurement legislation.
13 / 14
Bibliography
ISO 14025:2010. Environmental labels and declarations - Type III environmental declarations - Principles and procedures. International
Organization for Standardization.
ISO 14044:2006. Environmental management - Life cycle assessment - Requirements and guidelines. International Organization for
Standardization.
EN 15804:2012+A2:2019. Environmental product declaration - Core rules for the product category of construction products. European
Committee for Standardization.
ISO 21930:2017. Sustainability in buildings and civil engineering works - Core rules for environmental product declarations of construction
products. International Organization for Standardization.
EN 50693:2019. Product category rules for life cycle assessments of electronic and electrical products and systems. European Committee for
Standardization.
Ecoinvent v3, 2019. Allocation, cut-off by classification. Swiss Centre of Life Cycle Inventories.
Iversen et al., (2021). eEPD v2021.09, background information for EPD generator tool system verification, LCA.no. Report number: 07.21. System
verification report.
Babwah & Philis (2023). EPD generator based on PCR EPD Italy 007 with specific adaptation for electrical heaters, background information for EPD
generator application and LCA data, LCA.no. Report number 09.2023. PCR verification report (based on core PCR).
EPD Italy (2020). PCR EPD Italy 007 Part A for electronic and electrical products and systems. EPD Italy. Version 3, issue 13-01-2023 and valid
until 19-01-2025.
PEP Ecopassport (2023). PSR specific rules for direct, visible, fixed electric heating appliances. PSR-0002-ed3.0-EN-2023 06 06. Version 3, 06-06-
2023.
Program operator and publisher Phone: +47 977 22 020
The Norwegian EPD Foundation e-mail: post@epd-norge.no
Post Box 5250 Majorstuen, 0303 Oslo, Norway web: www.epd-norge.no
Owner of the declaration: Phone: +370 61579835
Adax AS e-mail: justinas.kulbe@adax.no
Myhres gate 1, 3060 Svelvik web: https://adax.no/
Author of the Life Cycle Assessment Phone: +47 916 50 916
LCA.no AS e-mail: post@lca.no
Dokka 6A, 1671 Kråkerøy web: www.lca.no
Developer of EPD generator Phone: +47 916 50 916
LCA.no AS e-mail: post@lca.no
Dokka 6A, 1671 Kråkerøy web: www.lca.no
ECO Platform web: www.eco-platform.org
ECO Portal web: ECO Portal
14 / 14
