ENVIRONMENTAL PRODUCT DECLARATION
as per ISO 14025 and EN 15804+A2
Owner of the Declaration Vitrulan Textile Glass GmbH
Publisher Institut Bauen und Umwelt e.V. (IBU)
Programme holder Institut Bauen und Umwelt e.V. (IBU)
Declaration number EPD-VIT-20230429-CBC1-EN
Issue date 09.01.2024
Valid to 08.01.2029
Nonwoven glass fibre wall covering
Vitrulan Textile Glass GmbH
www.ibu-epd.com | https://epd-online.com
General Information
Vitrulan Textile Glass GmbH Nonwoven glass fibre wall covering
Programme holder Owner of the declaration
IBU – Institut Bauen und Umwelt e.V. Vitrulan Textile Glass GmbH
Hegelplatz 1 Bernecker Straße 8
10117 Berlin 95509 Marktschorgast
Germany Germany
Declaration number Declared product / declared unit
EPD-VIT-20230429-CBC1-EN 1 m2 of nonwoven glass fibre wall covering with an average grammage of
around 0.124 kg/m2.
This declaration is based on the product category rules: Scope:
Wall coverings, 01.08.2021 This specific EPD document refers to nonwoven glass fibre wall covering
(PCR checked and approved by the SVR) produced by Vitrulan Textile Glass GmbH. The production data was
recorded in 2021. The production plant is located in Marktschorgast,
Germany.
Issue date
The owner of the declaration shall be liable for the underlying information
09.01.2024
and evidence; the IBU shall not be liable with respect to manufacturer
information, life cycle assessment data and evidences.
Valid to
The EPD was created according to the specifications of EN 15804+A2. In
08.01.2029 the following, the standard will be simplified as EN 15804.
Verification
The standard EN 15804 serves as the core PCR
Independent verification of the declaration and data according to ISO
14025:2011
internally X externally
Dipl.-Ing. Hans Peters
(Chairman of Institut Bauen und Umwelt e.V.)
Florian Pronold Vito D'Incognito,
(Managing Director Institut Bauen und Umwelt e.V.) (Independent verifier)
1 Environmental Product Declaration - Vitrulan Textile Glass GmbH - Nonwoven glass fibre wall covering
Product
the seam area must be avoided. Our nonwoven wall
Product description/Product definition coverings are suitable for double cutting.
Nonwoven glass fibre wall covering, manufactured by Vitrulan 4. PRESSING ON AND TRIMMING: Use a (hard plastic)
Textile Glass GmbH, is made of glass yarns and used for both, wallpaper spatula and press down firmly across the
functional and decorative purposes. It is generally distinguished entire length, smoothing out any air bubbles. Carefully
from wall paperings based on a paper substrate by a high- press (the) overlapping fabric into the corners and cut
quality special glass nonwoven which is used as the substrate with a sharp knife.
material. The glass fibre wall covering has a virtually seamless, 5. PAINTING: Apply the paint evenly, once the wall
uniform appearance. Generally, it is glued on walls and ceilings covering has completely dried. Follow the paint
and painted afterwards. It also includes white pigments to manufacturer's instructions. The need for further
reduce processing time on the construction site. It is particularly coatings depends on the paint quality, degree of gloss,
easy to handle: it does not shrink or stretch, is easy to cut and shade, expected stress, lighting situation and desired
produces perfect seams. It reinforces walls, covers smaller surface appearance. With raised fibres: Slight sanding
cracks, and prevents new smaller cracks from forming. between coatings is possible.
During application, the wall or ceiling is pasted and then the Technical Data
strip of wall covering is hung on the prepared paste bed, or, Main characteristics of our nonwoven glass fibre wall covering
alternatively, the wall covering comes with a water-activatable are:
adhesive which is already applied to the wall covering's backing
• Superb reaction to fire: B-s1, d0 according to DIN EN
– this adhesive then can be easily activated by water using the
13501-1
'Aqua-Quick device' specially developed for this purpose.
• Wall reinforcing and crack bridging: class A1 according
Vitrulan's Aqua Technology facilitates work and reduces
to Bundesausschuss Farbe und Sachwertschutz data
processing times for the user.
sheet (BFS-Merkblatt) No. 19
• Impact and perforation resistant
Since nonwoven glass fibre wall coverings are designed to
• Abrasion and scrub resistant (depending on the coating)
reinforce walls and ceilings, they are bonded to the building's
• Resistant to disinfectants and cleaning agents
structure. This means that they are disposed of as construction
(depending on the coating)
waste. Waste arising from installation can generally be
• Non-toxic and food-safe: OEKO-TEX-certified
disposed of as household waste since glass fibre wall
• Water vapour permeable
coverings are not classed as special waste. Our nonwoven wall
• Suitable for allergy sufferers
covering is OEKO-TEX-certified and completely non-hazardous
• In addition to the many technical benefits, nonwoven
to health. Sustainable interior design and premium product
glass fibre wall covering provides almost limitless scope
quality are hallmarks of all our textile glass wall coverings.
for creativity when it comes to interior design
For the placing on the market of the product in the European
Union/European Free Trade Association (EU/EFTA) (with the Constructional data
exception of Switzerland) Regulation (EU) No. 305/2011 (CPR) Name Value Unit
applies. The product needs a declaration of performance taking B-s1,
Fire behaviour according to EN 13501-1
into consideration EN 15102:2007+A1:2011 and the CE- d0
marking. For application and use, the respective national
Release of formaldehyde max. < 120 mg/kg
provisions apply. passed -
according to EN 12149
Application Migration of heavy metals (max.) and certain
passed -
other elements according to EN 12149
Nonwoven glass fibre wall coverings are used indoors on
ceilings and walls in the following steps. More details are to be Vinyl chloride monomer (VCM) content max.
passed -
found in the technical data sheets. < 0,2 mg/kg according to EN 12149
1. PREPARATION: Substrates should be dry, clean, Sound absorption according to ISO 354, ISO NPD -
smooth and stable. Pretreat absorbent substrates with a 11654
suitable primer. Do not apply with room and surface Thermal resistance according to EN 12667, EN
NPD -
temperatures below +8 °C. Use the same serial 12524
numbers when applying to adjacent areas. One drop =
wall height plus 5–10 cm.
Performance data of the product in accordance with the
2. APPLYING ADHESIVE: (a) Without Aqua Technology,
declaration of performance with respect to its essential
apply sufficient latex adhesive with a paint roller or
characteristics according to EN 15102:2007+A1:2011,
airless spray gun evenly to the wall over a width of 1–2
Decorative wall coverings – Roll and panel form.
sheets. Observe the adhesive manufacturer's
application notes. This also applies for applications with Base materials/Ancillary materials
a wall-papering device. (b) With Aqua Technology, the Our nonwoven glass fibre wall covering contains ca. 0.049
wall covering comes with a water-activatable adhesive kg/m2 raw glass fleece and ca. 0.075 kg/m2 coating based on
which is already applied to the wall covering's backing.
starch, polymeric materials and inorganic additives. It is
This adhesive can be easily activated by water using the
produced in two main phases.
'Aqua-Quick device'. At normal room
temperature/climate (18 °C, 60 %) the drying time is 12–
Raw glass fleece manufacture: The basic components of a
24 hours. When applicating under extreme climatic
glass batch are silica sand, limestone, kaolin, and boric acid.
conditions, the duration can change significantly.
These components are fused at approx. 1250˚C. The molten
3. BUTT-JOINING: Make sure that the edges butt up
glass flows by gravity through the nozzles of a bushing plate
smoothly where one length joins another. Overlaps in
2 Environmental Product Declaration - Vitrulan Textile Glass GmbH - Nonwoven glass fibre wall covering
made of platinum alloy to form filaments. A surface coating area, the picked wallpaper rolls are packaged individually
called a 'size' is applied to the individual filaments. The size before being sent for dispatch.
largely determines the processing characteristics of the glass
fibre material. The glass filaments are used to produce a raw According to the REACH regulation, these products are
glass fleece by means of a wetlaid production with chemical considered articles which do not fall under this regulation. With
bonding. regard to REACH, we can confirm that all raw materials we use
are registered and approved for use.
Product manufacture: The raw glass fleece is attributed to a
finishing treatment that completely coats the fleece. The finish These products contain substances listed in the Substances of
is normally applied using a special technique in which both Very High Concern candidate list (date: 15 June 2023)
sides of the unprocessed fleece are impregnated and then exceeding 0.1 percentage by mass: No.
dried. The finish determines essential product characteristics
such as stability, cutting capability, flexibility, feel, and surface Reference service life
roughness. Basically, the finish primes the surface optimally for The reference service life according to ISO 15686:1, -2, -7 and
subsequent application and painting. The finish for our pre- -8 are not indicated. The product is applied on internal walls
pigmented glass fleeces contains high-quality white pigments – and ceilings. Since it is designed to reinforce walls and ceilings,
this makes painting works on the construction site highly it is bonded to the building's structure. If well maintained, there
economical and significantly reduces labour and material costs. is no lifetime limitation. It creates the ideal substrate for
In the packing area, the dried and coated fleece is wound and decorative coatings and can be repainted over time and again
shortened in line with customer specifications. In the packaging without losing its performance.
LCA: Calculation rules
• Treatment of packaging material (A5) credits for
Declared Unit potential avoided burdens due to energy substitution of
The declared unit refers to 1 m2 of nonwoven glass fibre wall electricity and thermal energy generation are declared in
covering with an area weight of 0.124 kg/m². module D. Installation losses are also included in this
module.
Declared unit and mass reference
Name Value Unit
End-of-Life Stage - Modules C1-C4
Declared unit 1 m2
• Mechanical dismantling is considered (C1)
Grammage 0.124 kg/m2 • Transport to EoL (C2)
Layer thickness 0.00035 m • Disposal (C4) - landfill of the glass fibre wall covering
System boundary Benefits and Loads beyond product system boundary
No credits were accounted from the EoL scenario(C4) in
Type of EPD according to EN 15804: "cradle to gate with
module D. The credits in D are solely accounting for the
options, modules C1–C4, and module D". The following
avoided burdens calculated by the inversion of electricity grid
modules are declared: A1–A3, C, D and additional modules: A4
mix and thermal energy from natural gas during packaging
+ A5.
treatment (A5).
The following life cycle stages are considered:
Geographic Representativeness
Production - Modules A1-A3
Land or region, in which the declared product system is
The product stage includes:
manufactured, used or handled at the end of the product´s
• Raw material supply (A1): raw glass fleece and coating lifespan: Europe
based on starch besides polymeric materials and
inorganic additives
• Transport to the manufacturer (A2) Comparability
• Manufacturing (A3), including provision of all materials, Basically, a comparison or an evaluation of EPD data is only
products and energy, as well as waste processing up to possible if all the data sets to be compared were created
the end-of-waste state. according to EN 15804 and the building context, respectively
the product-specific characteristics of performance, are taken
Construction Stage - Modules A4- A5 into account. Sphera LCA FE (GaBi ts) serves as background
The construction process stage includes: database for the calculation. The CUP version 2022.2 is used.
• Transport to the construction site (A4)
LCA: Scenarios and additional technical information
Name Value Unit
Characteristic product properties of biogenic carbon
Biogenic carbon content in product (coating kg
For 1 m2 of nonwoven glass fibre wall covering, the biogenic 0.0056
based on starch) C
carbon content is declared below:
Biogenic carbon content in accompanying kg
0.00975
Information on describing the biogenic carbon content at packaging C
factory gate
Note: 1 kg of biogenic carbon is equivalent to 44/12 kg of CO .
2
3 Environmental Product Declaration - Vitrulan Textile Glass GmbH - Nonwoven glass fibre wall covering
Transport to the building site (A4)
Name Value Unit
End of life (C1-C4)
Litres of fuel 0.000299 l/100km
Name Value Unit
Transport distance 100 km
Collected separately waste type (send to landfill) 0.124 kg
Capacity utilisation (including empty runs) 50 %
Gross weight of product 0.124 kg
Reuse, recovery and/or recycling potentials (D), relevant
scenario information
For the thermal and electrical energy generated in Module A5
Installation into the building (A5) due to the packaging treatment, avoided burdens have been
The environmental results cover the cutting losses during calculated by the inversion of electricity grid mix and thermal
installation. The wall covering can come with/without aqua energy from natural gas, using European datasets and grouped
technology (self-adhesive layers). During application, the wall to Module D.
or ceiling is pasted and then the strip of wall covering is hung
on the prepared paste bed, or, alternatively, the wall covering
comes with a water-activatable adhesive which is already
applied to the wall covering's backing – this adhesive then can
be easily activated by water using the 'Aqua-Quick device'
specially developed for this purpose. Vitrulan's Aqua
Technology facilitates work and reduces processing times for
the user. The Public annexe to the EPD for the aqua technology
is declared in an attachment.
Name Value Unit
Material loss (Cuttings waste at installation) 0.00701 kg
Cardboard (waste packaging to incineration) 0.0134 kg/m2
Wooden pallets (waste packaging to
0.00804 kg/m2
incineration)
Polyethylene film (waste packaging to
0.001114kg/m2
incineration)
Paper (waste packaging to incineration) 0.00017 kg/m2
4 Environmental Product Declaration - Vitrulan Textile Glass GmbH - Nonwoven glass fibre wall covering
LCA: Results
The following table depicts the results of the indicators concerning the estimated impact, use of resources as well as waste and other
output flows in relation to 1 m² of nonwoven wall covering with the weight of 0.124 kg/m2.
DESCRIPTION OF THE SYSTEM BOUNDARY (X = INCLUDED IN LCA; MND = MODULE OR INDICATOR NOT DECLARED; MNR
= MODULE NOT RELEVANT)
Benefits and
Construction loads beyond
Product stage Use stage End of life stage
process stage the system
boundaries
la ire ta m w a Ry lp p u s tro p s n a rT g n iru tc a fu n a M e h t m o rf tro p s n a rTe tis e h t o t e ta g y lb m e s s A e s U e c n a n e tn ia M ria p e R tn e m e c a lp e R tn e m h s ib ru fe R y g re n e la n o ita re p Oe s u re ta w la n o ita re p Oe s u n o itc u rts n o c -e Dn o itilo m e d tro p s n a rT g n is s e c o rp e ts a W la s o p s iD -e s u e R-y re v o c e R-g n ilc y c e Rla itn e to p
A1 A2 A3 A4 A5 B1 B2 B3 B4 B5 B6 B7 C1 C2 C3 C4 D
X X X X X MND MND MNR MNR MNR MND MND X X X X X
RESULTS OF THE LCA - ENVIRONMENTAL IMPACT according to EN 15804+A2: 1 m2 Non-woven glass fibre wall covering
Parameter Unit A1-A3 A4 A5 C1 C2 C3 C4 D
GWP-total kg CO 2 eq 5.11E-01 9.17E-04 6.98E-02 1.28E-03 5.26E-04 0 2.24E-02 -6.43E-03
GWP-fossil kg CO 2 eq 5.61E-01 9.07E-04 3.63E-02 1.27E-03 5.2E-04 0 1.85E-03 -6.4E-03
GWP-biogenic kg CO 2 eq -5E-02 3.81E-06 3.34E-02 1.14E-05 2.18E-06 0 2.05E-02 -3.28E-05
GWP-luluc kg CO 2 eq 2.54E-04 6.23E-06 1.52E-05 2.69E-07 3.57E-06 0 3.42E-06 -7.04E-07
ODP kg CFC11 eq 2.17E-12 9.08E-17 1.27E-13 1.86E-14 5.21E-17 0 4.35E-15 -4.33E-14
AP mol H+ eq 2.2E-03 9.97E-07 1.33E-04 2.79E-06 6.27E-07 0 1.31E-05 -8.43E-06
EP-freshwater kg P eq 7.93E-06 3.3E-09 4.5E-07 3.71E-09 1.89E-09 0 3.14E-09 -8.82E-09
EP-marine kg N eq 4.41E-04 3.14E-07 2.8E-05 6.26E-07 2.08E-07 0 3.35E-06 -2.28E-06
EP-terrestrial mol N eq 4.73E-03 3.78E-06 3.08E-04 6.56E-06 2.48E-06 0 3.69E-05 -2.45E-05
kg NMVOC
POCP 1.32E-03 8.54E-07 8.28E-05 1.69E-06 5.44E-07 0 1.02E-05 -6.39E-06
eq
ADPE kg Sb eq 1.64E-07 9.32E-11 9.38E-09 3.46E-10 5.34E-11 0 1.9E-10 -9.67E-10
ADPF MJ 1.12E+01 1.21E-02 6.48E-01 2.3E-02 6.96E-03 0 2.42E-02 -1.09E-01
m3 world eq
WDP 1.83E-01 1.03E-05 1.48E-02 2.9E-04 5.93E-06 0 2.03E-04 -6.83E-04
deprived
GWP = Global warming potential; ODP = Depletion potential of the stratospheric ozone layer; AP = Acidification potential of land and water; EP =
Eutrophication potential; POCP = Formation potential of tropospheric ozone photochemical oxidants; ADPE = Abiotic depletion potential for non-fossil
resources; ADPF = Abiotic depletion potential for fossil resources; WDP = Water (user) deprivation potential)
RESULTS OF THE LCA - INDICATORS TO DESCRIBE RESOURCE USE according to EN 15804+A2: 1 m2 Non-woven glass
fibre wall covering
Parameter Unit A1-A3 A4 A5 C1 C2 C3 C4 D
PERE MJ 1.9E+00 8.41E-04 4.81E-01 1.28E-02 4.82E-04 0 3.64E-03 -2.99E-02
PERM MJ 3.51E-01 0 -3.51E-01 0 0 0 0 0
PERT MJ 2.25E+00 8.41E-04 1.3E-01 1.28E-02 4.82E-04 0 3.64E-03 -2.99E-02
PENRE MJ 1.12E+01 1.22E-02 6.96E-01 2.31E-02 6.99E-03 0 2.43E-02 -1.09E-01
PENRM MJ 4.79E-02 0 -4.79E-02 0 0 0 0 0
PENRT MJ 1.12E+01 1.22E-02 6.48E-01 2.31E-02 6.99E-03 0 2.43E-02 -1.09E-01
SM kg 1.06E-02 0 5.98E-04 0 0 0 0 0
RSF MJ 0 0 0 0 0 0 0 0
NRSF MJ 0 0 0 0 0 0 0 0
FW m3 7.58E-03 9.72E-07 5.34E-04 1.22E-05 5.57E-07 0 6.16E-06 -2.88E-05
PERE = Use of renewable primary energy excluding renewable primary energy resources used as raw materials; PERM = Use of renewable primary
energy resources used as raw materials; PERT = Total use of renewable primary energy resources; PENRE = Use of non-renewable primary energy
excluding non-renewable primary energy resources used as raw materials; PENRM = Use of non-renewable primary energy resources used as raw
materials; PENRT = Total use of non-renewable primary energy resources; SM = Use of secondary material; RSF = Use of renewable secondary fuels;
NRSF = Use of non-renewable secondary fuels; FW = Use of net fresh water
RESULTS OF THE LCA – WASTE CATEGORIES AND OUTPUT FLOWS according to EN 15804+A2:
1 m2 Non-woven glass fibre wall covering
Parameter Unit A1-A3 A4 A5 C1 C2 C3 C4 D
HWD kg 5.06E-09 6.45E-14 2.87E-10 1.99E-12 3.7E-14 0 1.25E-12 -1.47E-11
NHWD kg 9.36E-02 1.99E-06 1.31E-02 1.74E-05 1.14E-06 0 1.24E-01 -5.5E-05
RWD kg 3.47E-04 2.26E-08 2.02E-05 3.68E-06 1.3E-08 0 2.7E-07 -8.59E-06
CRU kg 0 0 0 0 0 0 0 0
MFR kg 0 0 0 0 0 0 0 0
MER kg 0 0 0 0 0 0 0 0
EEE MJ 0 0 3.05E-02 0 0 0 0 0
5 Environmental Product Declaration - Vitrulan Textile Glass GmbH - Nonwoven glass fibre wall covering
EET MJ 0 0 5.46E-02 0 0 0 0 0
HWD = Hazardous waste disposed; NHWD = Non-hazardous waste disposed; RWD = Radioactive waste disposed; CRU = Components for re-use;
MFR = Materials for recycling; MER = Materials for energy recovery; EEE = Exported electrical energy; EET = Exported thermal energy
RESULTS OF THE LCA – additional impact categories according to EN 15804+A2-optional:
1 m2 Non-woven glass fibre wall covering
Parameter Unit A1-A3 A4 A5 C1 C2 C3 C4 D
Disease
PM 2.28E-08 7.01E-12 1.34E-09 2.31E-11 4.17E-12 0 1.61E-10 -6.98E-11
incidence
IR kBq U235 eq 4.56E-02 3.42E-06 2.67E-03 6.24E-04 1.96E-06 0 2.99E-05 -1.45E-03
ETP-fw CTUe 3.77E+00 8.6E-03 2.19E-01 1.01E-02 4.93E-03 0 1.36E-02 -2.39E-02
HTP-c CTUh 1.52E-09 1.77E-13 8.62E-11 2.9E-13 1.02E-13 0 2.07E-12 -1.1E-12
HTP-nc CTUh 1.48E-07 9.58E-12 8.39E-09 1.06E-11 5.51E-12 0 2.3E-10 -4.22E-11
SQP SQP 9.26E+00 5.14E-03 5.27E-01 8.31E-03 2.95E-03 0 5.04E-03 -1.94E-02
PM = Potential incidence of disease due to PM emissions; IR = Potential Human exposure efficiency relative to U235; ETP-fw = Potential comparative
Toxic Unit for ecosystems; HTP-c = Potential comparative Toxic Unit for humans (cancerogenic); HTP-nc = Potential comparative Toxic Unit for humans
(not cancerogenic); SQP = Potential soil quality index
Disclaimer 1 – for the indicator “Potential Human exposure efficiency relative to U235”. This impact category deals mainly with the
eventual impact of low-dose ionizing radiation on human health of the nuclear fuel cycle. It does not consider effects due to possible
nuclear accidents, occupational exposure or radioactive waste disposal in underground facilities. Potential ionizing radiation from the
soil, radon and from some construction materials is also not measured by this indicator.
Disclaimer 2 – for the indicators “abiotic depletion potential for non-fossil resources”, “abiotic depletion potential for fossil resources”,
“water (user) deprivation potential, deprivation-weighted water consumption”, “potential comparative toxic unit for ecosystems”,
“potential comparative toxic unit for humans – cancerogenic”, “Potential comparative toxic unit for humans - not cancerogenic”,
“potential soil quality index”. The results of this environmental impact indicator shall be used with care as the uncertainties on these
results are high as there is limited experience with the indicator.
References
Standards ISO 15686
ISO 15686:1, -2, -7 and -8, Buildings and constructed assets —
EN 12149 Service life planning
DIN EN 12149, Wallcoverings in roll form - Determination of
migration of heavy metals and certain other elements, of vinyl Further References
chloride monomer and of formaldehyde release
Bundesausschuss Farbe und Sachwertschutz Merkblatt
EN 12524 No. 19
DIN EN 12524:2000, Building materials and products - BFS-Merkblatt No. 19, Risse in Außenputzen, Beschichtung
Hygrothermal properties - Tabulated design values und Armierung. Technical rules published by Bundesausschuss
Farbe und Sachwertschutz e.V.
EN 12667
DIN EN 12667:2001, Thermal performance of building materials IBU 2021
and products - Determination of thermal resistance by means of Institut Bauen und Umwelt e.V.: General Instructions for the
guarded hot plate and heat flow meter methods - Products of EPD programme of Institut Bauen und Umwelt e.V., Version
high and medium thermal resistance 2.0, Berlin: Institut Bauen und Umwelt e.V., 2021, www.ibu-
epd.com
EN 13501
EN 13501-1, Fire classification of construction products and OEKO-TEX
building elements - Part 1: Classification using test data from OEKO-TEX Standard 100, label for textiles tested for harmful
reaction to fire tests substances, https://www.oeko-tex.com/en/our-
standards/oekotex-standard-100 (accessed on 13 July 2023)
EN 15804
EN 15804:2012+A2:2019+AC:2021, Sustainability of PCR Part A
construction works — Environmental Product Declarations — PCR - Part A: Calculation rules for the Life Cycle Assessment
Core rules for the product category of construction products and Requirements on the Background Report, version 2.1,
Institut Bauen und Umwelt e.V.,2021
ISO 354
DIN EN ISO 354:2003, Acoustics - Measurement of sound PCR Part B
absorption in a reverberation room PCR – Part B: Requirements of the EPD for Wall coverings, v2,
Institut Bauen und Umwelt e.V., 2023
ISO 11654
DIN EN ISO 11654:1997, Acoustics - Sound absorbers for use REACH Regulation
in buildings - Rating of sound absorption REACH Regulation (EC) No 1907/2006 of the European
Parliament and of the Council of 18 December 2006 concerning
ISO 14025 the Registration, Evaluation, Authorisation and Restriction of
EN ISO 14025:2011, Environmental labels and declarations — Chemicals (REACH), establishing a European Chemicals
Type III environmental declarations — Principles and Agency, amending Directive 1999/45/EC and repealing Council
procedures. Regulation (EEC) No 793/93 and Commission Regulation (EC)
No 1488/94 as well as Council Directive 76/769/EEC and
6 Environmental Product Declaration - Vitrulan Textile Glass GmbH - Nonwoven glass fibre wall covering
Commission Directives 91/155/EEC, 93/67/EEC, 93/105/EC Sphera LCA FE (GaBi ts)
and 2000/21/EC GaBi ts dataset documentation for the software-system and
databases, LBP, University of Stuttgart and thinkstep,
Regulation No. 305/2011 Leinfelden-Echterdingen, 2023 (https://www.gabi-
Regulation (EU) No. 305/2011 of the European parliament and software.com/support/gabi)
of the Council of 9 March 2011 laying down harmonised
conditions for the marketing of construction products and SVHC list
repealing Council Directive 89/106/EEC EN Substances of Very High Concern candidate list (published in
15102:2007+A1:2011, Decorative wallcoverings - Roll and accordance with Article 59(10) of the REACH Regulation)
panel form products (accessed on 13 July 2023)
7 Environmental Product Declaration - Vitrulan Textile Glass GmbH - Nonwoven glass fibre wall covering
Publisher
Institut Bauen und Umwelt e.V. +49 (0)30 3087748- 0
Hegelplatz 1 info@ibu-epd.com
10117 Berlin www.ibu-epd.com
Germany
Programme holder
Institut Bauen und Umwelt e.V. +49 (0)30 3087748- 0
Hegelplatz 1 info@ibu-epd.com
10117 Berlin www.ibu-epd.com
Germany
Author of the Life Cycle Assessment
Sphera Solutions GmbH +49 711 341817-0
Hauptstraße 111- 113 info@sphera.com
70771 Leinfelden-Echterdingen www.sphera.com
Germany
Owner of the Declaration
Vitrulan Textile Glass GmbH +49 9227 77-0
Bernecker Straße 8 info@vitrulan.com
95509 Marktschorgast www.vitrulan.com
Germany
8 Environmental Product Declaration - Vitrulan Textile Glass GmbH - Nonwoven glass fibre wall covering
