ENVIRONMENTAL PRODUCT DECLARATION
as per ISO 14025 and EN 15804+A2
Owner of the Declaration Revigrés
Publisher Institut Bauen und Umwelt e.V. (IBU)
Programme holder Institut Bauen und Umwelt e.V. (IBU)
Declaration number EPD-REV-20240006-CCC1-EN
Issue date 22.03.2024
Valid to 21.03.2029
Glazed and unglazed porcelain tiles
Revigrés
www.ibu-epd.com | https://epd-online.com
General Information
Revigrés Glazed and unglazed porcelain tiles
Programme holder Owner of the declaration
IBU – Institut Bauen und Umwelt e.V. Revigrés
Hegelplatz 1 Apartado 1 Barrô
10117 Berlin 3754 Águeda
Germany Portugal
Declaration number Declared product / declared unit
EPD-REV-20240006-CCC1-EN Glazed and Unglazed Porcelain Tiles/1 m2 of ceramic tiles
This declaration is based on the product category rules: Scope:
Ceramic tiles and panels, 01.08.2021 The EPD applies to 1m² of glazed and unglazed porcelain tiles, produced
(PCR checked and approved by the SVR) by Revigrés, in its facilities located in Barrô - Águeda - Aveiro - Portugal.
The results presented correspond to an average EPD of the Revigrés.
The owner of the declaration shall be liable for the underlying information
Issue date and evidence; the IBU shall not be liable with respect to manufacturer
information, life cycle assessment data and evidences.
22.03.2024
The EPD was created according to the specifications of EN 15804+A2. In
the following, the standard will be simplified as EN 15804.
Valid to
21.03.2029 Verification
The standard EN 15804 serves as the core PCR
Independent verification of the declaration and data according to ISO
14025:2011
internally X externally
Dipl.-Ing. Hans Peters
(Chairman of Institut Bauen und Umwelt e.V.)
Florian Pronold Mr Olivier Muller,
(Managing Director Institut Bauen und Umwelt e.V.) (Independent verifier)
1 Environmental Product Declaration - Revigrés - Glazed and unglazed porcelain tiles
Product
Name Value Unit
Product description/Product definition
Deviation of mean thickness from
The Revigrés glazed and unglazed porcelain tiles are produced ± 0.5% max ±
manufacturing thickness (ISO 10545- --
combining technological innovation with good environmental 0.5 mm
2)
practices.
%
Water Absorption (ISO 10545-3) < 0.1
(W/W)
They are dry pressed and characterized by technical
specifications (high mechanical strength and resistance to Bending Strength thickness < 7.5 mm
> 700 N
wear, chemical and stains), and it is fully vitrified (at (ISO 10545-4)
temperature of over 1200 ºC) acquiring extremely low water Bending Strength thickness ≥ 7.5 mm
≥ 1300 N
absorption, no more than 0.5%, with consequently frost (ISO 10545-4)
resistance, making it suitable for outdoor installation. Rupture Modulus (ISO 10545-4) > 45 N/mm2
Test method
In porcelain tiles, each series can have different dimensions, Impact resistance (ISO 10545-5) --
available
colours, textures and finishes:
Deep abrasion (unglazed tiles) (ISO
• Edge: natural and rectified; < 120 mm3
10545-6)
• Surface: such as matte, glossy, non-slip, softened and
Resistance to surface abrasion PEI GROUPS
polished. --
(glazed tiles) (ISO 10545-7) 1-2-3-4-5
and thanks to its superior technical characteristics, allows the
Designer to satisfy all project requirements. For the placing on Cracking Resistance (glazed tiles) Resistant --
the market of the product in the European Union/European (ISO 10545-11)
Free Trade Association (EU/EFTA) (with the exception of Coefficient of Linear Thermal
Switzerland) Regulation (EU) No. 305/2011 (CPR) applies. The expansion (with atmospheric
≤ 8,0x10^-6 / °C
product needs a Declaration of Performance taking into temperature up to 100 °C) (ISO
consideration /EN 14411:2012 Ceramic tiles — Definitions, 10545-8)
classification, characteristics, evaluation of conformity and Resistant to frost (ISO 10545-12) Resistant --
marking/ and the CE-marking.
Resistance to thermal shock (ISO
For the application and use the respective national provisions Resistant --
10545-9)
apply.
Resistance to Acids and low
from LA to LB --
Application concentrations Bases (ISO 10545-13)
Ceramic Porcelain tiles can be applied both indoor and outdoor Resistance to Acids and high
from HA to HB --
areas: concentrations Bases (ISO 10545-13)
Resistance to household chemicals
• indoor/outdoor covering
ans swimming pool water additives Min. class B --
• floor/wall covering
(ISO 10545-13)
• commercial buildings
• residential buildings Resistance to staining (ISO 10545-14) Min. class 3 --
• industrial buildings To be
Antislip Resistance - pendulum test
• floors of outdoor facilities such as gardens, terraces, confirmed case --
value (ENV 12633)
pool sides and recreational areas by case
To be
Technical Data Antislip Resistance - shod ramp test
confirmed case --
The Revigrés porcelain tiles comply with requirements of (DIN EN 16165 annexe b)
by case
standard of EN 14411:2012 Group Bla (dry-pressed with water
To be
absortion E<0.5%), and ISO 10545 standards Antislip Resistance - barefoot ramp
confirmed case --
For each product, the data provided in the Declaration of test (DIN EN 16165 annexe a)
by case
Performance applies.
To be
Antislip Resistance - pendulum test
Most relevant technical characteristics: value - 4S (DIN EN 16165 annexe c) confirmed case --
by case
Constructional data
To be
Antislip Resistance (DCOF) (ANSI A
confirmed case --
326.3)
by case
Reaction to fire (EN 13823 . EN 9239-
A1FL --
1)
• Performance data of the product in accordance with the
declaration of performance with respect to its essential
characteristics according to EN 14411:2012 (Group BIa
GL or UGL), Ceramic tiles - Definition, classification,
characteristics, assessment and verification of
constancy of performance and marking.
Base materials/Ancillary materials
Ceramic tiles are mainly made of raw natural material such as
clay, kaolin, feldspar, silica sand. The finishing product includes
frits, pigments, binders, and other auxiliary
2 Environmental Product Declaration - Revigrés - Glazed and unglazed porcelain tiles
substances/additives like dispersant, pigment, binder and
rheological additives. Reference service life
The life cycle duration was based on product standard EN
Name Value Unit
14411 and annexe H of NF EN 15804+A2+ AC/CN.
Clay 40 - 43 %
According to EN 17160, PCR of this product, which is based on
Kaolin 5 - 7 % EN 14411:2012 (Ceramic tiles - Definitions, classification,
Feldspar 46 - 49 % characteristics, conformity assessment and marking), the
Silica sand 5 - 8 % reference life of the product is estimated at 50 years (Table H.2
— List of default DVRs by product category). No repair, renewal
Others 0 - 2 %
or replacement is necessary during this lifetime.
LCA: Calculation rules
Declared Unit Geographic Representativeness
1 m2 of glazed and unglazed porcelain tiles. Land or region, in which the declared product system is
manufactured, used or handled at the end of the product´s
Declared unit and mass reference
lifespan: Global
Name Value Unit
Declared unit 1 m2
Comparability
Grammage 19.8 kg/m2
Basically, a comparison or an evaluation of EPD data is only
conversion factor [Mass/Declared Unit] 0.0505 -
possible if all the data sets to be compared were created
Layer thickness 0.0083 m according to EN 15804 and the building context, respectively
the product-specific characteristics of performance, are taken
System boundary into account. The Ecoinvent v3.7.1 background database has
Type of the EPD: cradle to grave. been used to calculate the EPD results.
LCA: Scenarios and additional technical information
Use or application of the installed product (B1) see section
Characteristic product properties of biogenic carbon
2.12 "Use"
The product does not contain biogenic carbon.
Packaging material contains biogenic carbon that is accounted Name Value Unit
for in this section. According to EN 17160 and IBU PCR - Part B ceramic tiles are
Information on describing the biogenic carbon content at intrinsically inert and therefore do not have environmental
factory gate impacts during their use to be addressed in module B1.
Name ValueUnit
kg Maintenance (B2)
Biogenic carbon content in product -
C Name Value Unit
Biogenic carbon content in accompanying kg Information on Cleaning 52 times per year
0.185 -
packaging C maintenance (residential use)
Note: 1 kg biogenic Carbon is equivalent to 44/12 kg of CO . Maintenance cycle 2600 Number/RSL
2
Water consumption 0.26 m3
Detergent
0.53 l
The following information refers to the declared modules and is consumprtion
the basis for calculations or can beused for further calculations.
The indicated values refer to the declared unit.
In case a reference service life according to applicable ISO
Transport to the building site (A4) standards is declared then the assumptions and in-use
Name Value Unit conditions underlying the determined RSL shall be declared. In
addition, it shall be stated that the RSL applies to the reference
Transport distance 1390 km
conditions only.
Capacity utilisation (including empty runs) < 100 %
Gross density of products transported 270 kg/m3 The same holds for a service life declared by the manufacturer.
This scenario is based on EN 17160 and IBU PCR - Part B. Corresponding information related to in-use conditions needs
not be provided if a service life taken from the list of service life
by BNB is declared.
Installation into the building (A5)
Name Value Unit
Reference service life
Auxiliary (cement mortar) 3.3 kg
Name ValueUnit
Water consumption 0.0008 m3
Reference service life (according to ISO 15686-1, -
Material loss 0.595 kg 2, -7 and -8) 50 a
Wood pallets 0.529 kg
End of life (C1-C4)
Paper waste 0.043 kg
Plastic waste 0.023 kg Name Value Unit
Waste for recycling 16.19 kg
This scenario is based on EN 17160 and IBU PCR - Part B.
Waste for landfilling 6.94 kg
3 Environmental Product Declaration - Revigrés - Glazed and unglazed porcelain tiles
This scenario is based on EN 17160 and IBU PCR - Part B. asphalt (Silvestre et al., 2013);
• recycled ceramic aggregates can be used in the
construction of landfills;
Reuse, recovery and/or recycling potentials (D), relevant
• recycled ceramic aggregates can be utilized in the
scenario information
construction of subbased courses on secondary roads
After the demolition/deconstruction stage, ceramic tiles can be
crushed and then used in a range of different applications such
In this case, the modelling was carried out based on the
as describer in EN 17160 and IBU PCR - Part B:
replacement of natural aggregates (70%).
• recycled ceramic aggregates which can be integrated as
Name Value Unit
a partial substitute of natural aggregate in hotmix
4 Environmental Product Declaration - Revigrés - Glazed and unglazed porcelain tiles
LCA: Results
DESCRIPTION OF THE SYSTEM BOUNDARY (X = INCLUDED IN LCA; MND = MODULE OR INDICATOR NOT DECLARED; MNR
= MODULE NOT RELEVANT)
Benefits and
Construction loads beyond
Product stage Use stage End of life stage
process stage the system
boundaries
la ire ta m w a Ry lp p u s tro p s n a rT g n iru tc a fu n a M e h t m o rf tro p s n a rTe tis e h t o t e ta g y lb m e s s A e s U e c n a n e tn ia M ria p e R tn e m e c a lp e R tn e m h s ib ru fe R y g re n e la n o ita re p Oe s u re ta w la n o ita re p Oe s u n o itc u rts n o c -e Dn o itilo m e d tro p s n a rT g n is s e c o rp e ts a W la s o p s iD -e s u e R-y re v o c e R-g n ilc y c e Rla itn e to p
A1 A2 A3 A4 A5 B1 B2 B3 B4 B5 B6 B7 C1 C2 C3 C4 D
X X X X X X X MNR MNR MNR MND MND X X X X X
RESULTS OF THE LCA - ENVIRONMENTAL IMPACT according to EN 15804+A2: 1 m2 Glazed and unglazed porcelain tiles
Parameter Unit A1-A3 A4 A5 B1 B2 C1 C2 C3 C4 D
GWP-total kg CO 2 eq 1.35E+01 3.72E+00 1.77E+00 0 8.3E-01 0 1.34E-01 1.04E-01 5.77E-02 -2.85E-02
GWP-fossil kg CO 2 eq 1.39E+01 3.72E+00 1.11E+00 0 8.09E-01 0 1.34E-01 1.03E-01 5.76E-02 -2.67E-02
GWP-
biogenic kg CO 2 eq -4.8E-01 2.97E-03 6.61E-01 0 2.04E-02 0 1.07E-04 1.59E-03 1.67E-04 -1.76E-03
GWP-luluc kg CO 2 eq 2.46E-02 2.82E-05 8.28E-04 0 4.46E-04 0 1.01E-06 5.02E-05 1.29E-06 -1.57E-05
ODP kg CFC11 eq 2.85E-06 8.64E-07 1.13E-07 0 8.99E-08 0 3.11E-08 1.88E-08 1.3E-08 -4.95E-09
AP mol H+ eq 4.17E-02 7.33E-03 3.36E-03 0 5.54E-03 0 2.64E-04 9.14E-04 5.18E-04 -2.28E-04
EP-
kg P eq 1.89E-04 2.03E-06 1.65E-05 0 3.05E-05 0 7.3E-08 2.51E-06 6.11E-08 -6.29E-07
freshwater
EP-marine kg N eq 1.22E-02 1.22E-03 9.67E-04 0 7.5E-04 0 4.4E-05 3.66E-04 2.26E-04 -9.1E-05
EP-terrestrial mol N eq 9.96E-02 1.36E-02 9.46E-03 0 8.22E-03 0 4.9E-04 4.02E-03 2.48E-03 -1E-03
kg NMVOC
POCP 4.12E-02 4.81E-03 2.96E-03 0 3.66E-03 0 1.73E-04 1.1E-03 6.73E-04 -2.77E-04
eq
ADPE kg Sb eq 7.01E-04 1.58E-07 2.1E-05 0 3.73E-07 0 5.68E-09 4.6E-09 2.76E-09 -7.65E-09
ADPF MJ 2.03E+02 5.27E+01 9.79E+00 0 2.83E+01 0 1.9E+00 1.57E+00 8.04E-01 -5.46E-01
m3 world eq
WDP 4.5E+00 -1.12E-02 1.6E-01 0 1.16E+01 0 -4.02E-04 4.84E-03 1.29E-04 -8.2E-03
deprived
GWP = Global warming potential; ODP = Depletion potential of the stratospheric ozone layer; AP = Acidification potential of land and water; EP =
Eutrophication potential; POCP = Formation potential of tropospheric ozone photochemical oxidants; ADPE = Abiotic depletion potential for non-fossil
resources; ADPF = Abiotic depletion potential for fossil resources; WDP = Water (user) deprivation potential)
RESULTS OF THE LCA - INDICATORS TO DESCRIBE RESOURCE USE according to EN 15804+A2: 1 m2 Glazed and unglazed
porcelain tiles
Parameter Unit A1-A3 A4 A5 B1 B2 C1 C2 C3 C4 D
PERE MJ 3.67E+01 7.76E-02 1.87E+00 0 5.65E-01 0 2.79E-03 8.58E-02 1.46E-02 -1.99E-01
PERM MJ 2.22E-04 0 2.19E-01 0 0 0 0 0 0 0
PERT MJ 3.67E+01 7.76E-02 2.09E+00 0 5.65E-01 0 2.79E-03 8.58E-02 1.46E-02 -1.99E-01
PENRE MJ 2.22E+02 5.6E+01 1.06E+01 0 3.02E+01 0 2.01E+00 1.67E+00 8.59E-01 -5.7E-01
PENRM MJ 2.37E-05 0 0 0 0 0 0 0 0 0
PENRT MJ 2.22E+02 5.6E+01 1.06E+01 0 3.02E+01 0 2.01E+00 1.67E+00 8.59E-01 -5.7E-01
SM kg 6.48E-01 0 0 0 0 0 0 0 0 0
RSF MJ 0 0 0 0 0 0 0 0 0 0
NRSF MJ 0 0 0 0 0 0 0 0 0 0
FW m3 1.13E-01 1.05E-03 6.53E-03 0 2.72E-01 0 3.76E-05 4.04E-04 4.75E-05 -4.81E-03
PERE = Use of renewable primary energy excluding renewable primary energy resources used as raw materials; PERM = Use of renewable primary
energy resources used as raw materials; PERT = Total use of renewable primary energy resources; PENRE = Use of non-renewable primary energy
excluding non-renewable primary energy resources used as raw materials; PENRM = Use of non-renewable primary energy resources used as raw
materials; PENRT = Total use of non-renewable primary energy resources; SM = Use of secondary material; RSF = Use of renewable secondary fuels;
NRSF = Use of non-renewable secondary fuels; FW = Use of net fresh water
RESULTS OF THE LCA – WASTE CATEGORIES AND OUTPUT FLOWS according to EN 15804+A2:
1 m2 Glazed and unglazed porcelain tiles
Parameter Unit A1-A3 A4 A5 B1 B2 C1 C2 C3 C4 D
HWD kg 2.21E-03 1.4E-04 7.07E-05 0 1.43E-05 0 5.03E-06 2.99E-06 2.11E-06 -7.93E-07
NHWD kg 1.83E+00 2.21E-03 2.94E-01 0 2.47E-02 0 7.93E-05 2.42E+00 6.93E+00 -6.5E-04
RWD kg 3.94E-04 3.82E-04 3.37E-05 0 1.88E-05 0 1.38E-05 1.12E-05 5.86E-06 -5.01E-06
CRU kg 0 0 0 0 0 0 0 0 0 0
MFR kg 2.53E-02 0 6.6E-01 0 0 0 0 1.62E+01 0 0
MER kg 7.39E-03 0 1.68E-01 0 0 0 0 0 0 0
EEE MJ 1.55E+00 0 3.2E+01 0 0 0 0 0 0 0
5 Environmental Product Declaration - Revigrés - Glazed and unglazed porcelain tiles
EET MJ 0 0 0 0 0 0 0 0 0 0
HWD = Hazardous waste disposed; NHWD = Non-hazardous waste disposed; RWD = Radioactive waste disposed; CRU = Components for re-use;
MFR = Materials for recycling; MER = Materials for energy recovery; EEE = Exported electrical energy; EET = Exported thermal energy
RESULTS OF THE LCA – additional impact categories according to EN 15804+A2-optional:
1 m2 Glazed and unglazed porcelain tiles
Parameter Unit A1-A3 A4 A5 B1 B2 C1 C2 C3 C4 D
Disease
PM 9.5E-07 2.14E-07 5.29E-08 0 5.17E-08 0 7.71E-09 8.47E-08 4.04E-08 -6.05E-09
incidence
IR kBq U235 eq 3.18E-01 2.32E-01 3.46E-02 0 2E-02 0 8.36E-03 8.9E-03 3.55E-03 -6.34E-03
ETP-fw CTUe 1.42E+02 2.11E+01 1.01E+01 0 1.26E+01 0 7.58E-01 5.92E-01 3.05E-01 -2.68E-01
HTP-c CTUh 6.87E-09 2.78E-10 3.33E-10 0 2.77E-09 0 9.99E-12 1.06E-11 6.26E-12 -2.06E-11
HTP-nc CTUh 2.15E-07 3.3E-08 1.16E-08 0 2.76E-08 0 1.19E-09 6.84E-10 4.21E-10 -2.22E-10
SQP SQP 1.58E+02 1.68E-01 1.23E+01 0 1.37E+00 0 6.04E-03 4.75E-01 2.96E-01 -9.3E-01
PM = Potential incidence of disease due to PM emissions; IR = Potential Human exposure efficiency relative to U235; ETP-fw = Potential comparative
Toxic Unit for ecosystems; HTP-c = Potential comparative Toxic Unit for humans (cancerogenic); HTP-nc = Potential comparative Toxic Unit for humans
(not cancerogenic); SQP = Potential soil quality index
Disclaimer 1 – for the indicator “Potential Human exposure efficiency relative to U235”. This impact category deals mainly with the
eventual impact of low-dose ionizing radiation on human health of the nuclear fuel cycle. It does not consider effects due to possible
nuclear accidents, occupational exposure or radioactive waste disposal in underground facilities. Potential ionizing radiation from the
soil, radon and from some construction materials is also not measured by this indicator.
Disclaimer 2 – for the indicators “abiotic depletion potential for non-fossil resources”, “abiotic depletion potential for fossil resources”,
“water (user) deprivation potential, deprivation-weighted water consumption”, “potential comparative toxic unit for ecosystems”,
“potential comparative toxic unit for humans – cancerogenic”, “Potential comparative toxic unit for humans - not cancerogenic”,
“potential soil quality index”. The results of this environmental impact indicator shall be used with care as the uncertainties on these
results are high as there is limited experience with the indicator.
References
ANSI A 326.3 IBU
ANSI A326.3-2021. Dynamic Coefficient Of Friction (DCOF) Of Institut Bauen und Umwelt e.V.: General Instructions for the
Hard Surface Flooring Materials EPD programme of Institut Bauen und Umwelt e.V., Version
2.0, Berlin: Institut Bauen und Umwelt e.V., 2021
CRP www.ibu-epd.com.
Regulation (EU) No. 305/2011 of the European Parliament and
of the Council of 9 March 2011 laying down harmonised IBU PCR Part AInstitut Bauen und Umwelt e.V. (IBU): Product
conditions for the marketing of construction products and Category Rules for Building-Related Products and Services |
repealing Council Directive 89/106/EEC Part A: Calculation Rules for the Life Cycle Assessment and
Requirements on the Project Report, Version 2.2, Berlin Institut
DIN 51130 Bauen und Umwelt e.V., 2022
DIN 51130: 2023-03. Testing of floor coverings - Determination
of the displacement space IBU PCR Part B
Institut Bauen und Umwelt e.V. (IBU): Product Category Rules
EN 13823 for Building-Related Products and Services | Part B:
EN 13823:2020+A1:2022. Reaction to fire tests for building Requirements on the EPD for Ceramic tiles and panels, v5,
products - Building products excluding floorings exposed to the 11.07.2023
thermal attack by a single burning item
ISO 10545-2
EN 14411 ISO 10545-2:2018. Ceramic tiles – Part 2: Determination of
EN 14411:2012. Ceramic tiles. Definitions, classification, dimensions and surface quality
characteristics, evaluation of conformity and marking. Brussels,
Belgium. ISO 10545-3
ISO 10545-3:2018. Ceramic tiles – Part 3: Determination of
EN 15804 water absorption, apparent porosity, apparent relative density
EN 15804:2012+A2:2019+AC:2021, Sustainability of and bulk density
construction works — Environmental Product D
eclarations — Core rules for the product category of ISO 10545-4
construction products. ISO 10545-4:2019. Ceramic tiles – Part 4: Determination of
modulus of rupture and breaking strength
EN ISO 14025
EN ISO 14025:2011, Environmental labels and declarations — ISO 10545-5
Type III environmental declarations — Principles and ISO 10545-5:1996. Ceramic tiles - Part 5: Determination of
procedures. impact resistance by measurement of coefficient of restitution
EN 14411 ISO 10545-6
EN 14411:2012. Ceramic tiles. Definitions, classification, ISO 10545-6:2010. Ceramic tiles – Part 6: Determination of
characteristics, evaluation of conformity and marking. Brussels, resistance to deep abrasion for unglazed tiles
Belgium
6 Environmental Product Declaration - Revigrés - Glazed and unglazed porcelain tiles
ISO 10545-7 ISO 10545-14
ISO 10545-7:1996. Ceramic tiles – Part 7: Determination of ISO 10545-14:2015. Ceramic tiles – Part 14: Determination of
resistance to surface abrasion for glazed tiles resistance to stains
ISO 10545-8 ISO 13006
ISO 10545-8:2014. Ceramic tiles – Part 8: Determination of ISO 13006: 012. Ceramic tiles - Definitions, classification,
linear thermal expansion characteristics and marking, 2nd edn. International
Organization for Standardization, USA
ISO 10545-9
ISO 10545-9:2013. Ceramic tiles – Part 9: Determination of Regulation (EU) No. 305/2011
resistance to thermal shock Regulation (EU) No. 305/2011 of the European Parliament and
of the Council of 9 March 2011 laying down harmonised
ISO 10545-11 conditions for the marketing of construction products and
ISO 10545-11:1994. Ceramic tiles – Part 11: Determination of repealing Council Directive 89/106/EEC
crazing resistance for glazed tiles
SimaProSimaPro/ SimaPro LCA Software. Pré Consultants. the
ISO 10545-12 Netherlands. www.presustainability.com
ISO 10545-12:1995. Ceramic tiles – Part 12: Determination of
frost resistance The literature referred to in the Environmental Product
Declaration must be listed in full.Standards already fully quoted
ISO 10545-13 in the EPD do not need to be listed here again.
ISO 10545-13:2016. Ceramic tiles – Part 13: Determination of The current version of PCR Part A and PCR Part B of the PCR
chemical resistance document on which they are based must be referenced.
7 Environmental Product Declaration - Revigrés - Glazed and unglazed porcelain tiles
Publisher
Institut Bauen und Umwelt e.V. +49 (0)30 3087748- 0
Hegelplatz 1 info@ibu-epd.com
10117 Berlin www.ibu-epd.com
Germany
Programme holder
Institut Bauen und Umwelt e.V. +49 (0)30 3087748- 0
Hegelplatz 1 info@ibu-epd.com
10117 Berlin www.ibu-epd.com
Germany
Author of the Life Cycle Assessment
Centro Tecnológico da Cerâmica e do Vidro +351 239499200
iParque Lote 6 marisa@ctcv.pt
3040-540 Antanhol www.ctcv.pt
Portugal
Owner of the Declaration
Revigrés +351 234 660 100
Apartado 1 Barrô revigres@revigres.pt
3754 Águeda www.revigres.pt
Portugal
8 Environmental Product Declaration - Revigrés - Glazed and unglazed porcelain tiles
