ENVIRONMENTAL PRODUCT DECLARATION
as per ISO 14025 and EN 15804+A2
Owner of the Declaration Gradus Ltd.
Publisher Institut Bauen und Umwelt e.V. (IBU)
Programme holder Institut Bauen und Umwelt e.V. (IBU)
Declaration number EPD-SHA-20230476-CBA3-EN
Issue date 18/12/2023
Valid to 17/12/2028
Gradus Carpet Tile with Nylon Face Fibre
Gradus Ltd.
www.ibu-epd.com | https://epd-online.com
General Information
Gradus Ltd. Gradus Carpet Tile with Nylon Face Fibre
Programme holder Owner of the declaration
IBU – Institut Bauen und Umwelt e.V. Gradus Ltd.
Hegelplatz 1 Chapel Mill, Park Green *
10117 Berlin SK11 7LZ Mecclesfield, Cheshire
Germany United Kingdom
Declaration number Declared product / declared unit
EPD-SHA-20230476-CBA3-EN 1 m2 of installed Gradus Bitumen Backed Carpet Tile
This declaration is based on the product category rules: Scope:
Floor coverings, 01/08/2021 A Life Cycle Assessment (LCA) was conducted based upon production
(PCR checked and approved by the SVR) data collected from Gradus, Ltd. manufacturing facility (Chapel Mill, Park
Green, Macclesfield, Cheshire, SK11 7LZ), located in Scotland, UK.
Production data was collected for Gradus Premium Loop Pile Tufted,
Issue date Bitumen Backed Carpet Tile with Nylon Face Fibre, for the period of one
year, from January to December 2021.
18/12/2023
This EPD is cradle-to-gate with options in scope with additional modules
A4, A5, B1 and B2. The EPD is created in accordance to the specifications
Valid to
of EN 15804+A2.
17/12/2028
The functional unit has been defined as 1 m2 of installed Gradus Premium
Loop Pile Tufted, Bitumen Backed Carpet Tile.
The EPD was generated with the help of Envision LCA Tool, version 1. The
tool has not been manipulated in calculating impact results. The current
version of the tool is maintained, saved, and stored for 10 years to be used
for revision and re-traceability purposes.
The owner of the declaration shall be liable for the underlying information
and evidence; the IBU shall not be liable with respect to manufacturer
information, life cycle assessment data and evidences.
Dipl.-Ing. Hans Peters The EPD was created according to the specifications of EN 15804+A2. In
(Chairman of Institut Bauen und Umwelt e.V.) the following, the standard will be simplified as EN 15804.
Verification
The standard EN 15804 serves as the core PCR
Independent verification of the declaration and data according to ISO
14025:2011
internally X externally
Florian Pronold Mrs Kim Allbury,
(Managing Director Institut Bauen und Umwelt e.V.) (Independent verifier)
1 Environmental Product Declaration - Gradus Ltd. - Gradus Carpet Tile with Nylon Face Fibre
Product
product meets the requirements of the harmonized European
Product description/Product definition Norm (hEN): EN14041:2004A/C:2006. Declarations of
This EPD applies to Gradus Premium Loop Pile Tufted, performance related to fire, electrostatic, formaldehyde
Bitumen Backed Carpet Tile with Nylon face fibre. emissions, and slip resistance can be found on the product's
specification sheet.
The carpet tile backing system contains a modified bitumen
Constructional data
polymer, mineral filler, and a fibreglass reinforcement layer for
dimensional stability. The face fibre is made of solution-dyed Name Value Unit
Nylon that is tufted into a primary backing sheet, then latex is Product thickness 5.8 - 6.2 mm
added to anchor the fibre in place to assure maximum tuft bind. Grammage 3896.4 g/m2
The bitumen-based backing system is then applied to create a
Product Form Carpet Tile -
durable flooring solution for use in varied applications. The
Yarn type - Solution-dyed 0% Post-industrial
carpet tiles are then die-cut and packaged for distribution. -
Nylon 6 Recycled Content
This Gradus Premium Loop Pile Tufted, Bitumen Backed Total thickness 5.8 - 6.2 mm
Carpet Tile is a commercial carpet tile, suitable for use in all Total carpet weight 3600 - 4170 g/m2
commercial settings as a floor covering, in accordance with
Surface pile thickness 2.4 - 2.6 mm
manufacturer guidelines. It has a life span of 12 years and
Surface pile weight - Nominal
comes with a 12-year wear warranty (subject only to installation 610 - 800 g/m2
Pile Mass
and maintenance being carried out in line with manufacturer's
Length and width of squared
guidelines). The product meets both internal and external 250 - 1000 mm
elements
performance standards including those established in the EU
under EN 1307 and EN 10874 for a product suitable for heavy Other technical data parameters listed in IBU PCR Part B are
and general commercial installations. not relevant and, therefore, have not been declared.
This product is manufactured in the UK. Raw materials are Performance data of the product in accordance with the
responsibly sourced through supply chain, chemical and waste declaration of performance with respect to its essential
management programs. No co-products are produced in the characteristics according to 14041:2004A/C:2006.
manufacturing of these premium carpet tiles.
Base materials/Ancillary materials
Detailed Product Descriptions: Gradus Premium Loop Pile Tufted, Bitumen Backed Carpet Tile
with Nylon Face Fibre is comprised of the following raw
Urban Myth is a textured loop pile carpet available in both tile materials:
and plank format. The random design offers versatility and the
• 50-60% Calcium Carbonate Filler
opportunity to create innovative and complimentary colours
• 12-18% Modified Bitumen Polymer
comprising six grey base tones and six vibrant accent colours
• 12-18% Solution-dyed Nylon 6 Face Fibre
that can be combined to create stunning installations.
• 8-13% Styrene Butadiene Co-Polymer Latex
• 1-4% Polyester Primary Backing
Lunar is a tufted loop pile carpet tile. Inspired by the lunar
• 1-3% Polypropylene Secondary Backing
landscape, the design is available in a choice of eight
• 0.1-1% Fibreglass Reinforcement
colourways to help create a stylish and modern environment.
• 0-0.1% Anti-stat
Lunar is suitable for use in a wide range of applications
The product is packaged in cardboard boxes, wrapped in
including commercial office and education spaces.
plastic, and stacked on wooden pallets for distribution.
Cityscene & Brickworks are tufted loop pile carpet tiles that can
The product fits into the defined scope and all raw material
be used together to create interesting and contemporary floor
inputs, with no exceptions, are captured by the Envision LCA
schemes. They can also be combined with Emphasis to create
Tool, version 1.
a unique design statement. They are suitable for a wide range
of uses including commercial office, education, and healthcare.
This product contains substances listed in the candidate list
For the placing on the market of the product in the European
(date: 17.01.2023) exceeding 0.1 percentage by mass: no
Union/European Free Trade Association (EU/EFTA) (with the
exception of Switzerland) Regulation (EU) No. 305/2011 (CPR)
This product contains other CMR substances in categories 1A
applies. The product needs a declaration of performance taking
or 1B which are not on the candidate list, exceeding 0.1
into consideration EN 14041:2004A/C:2006, and the CE-
percentage by mass: no
marking.
Biocide products were added to this construction product or it
For the application and use, the respective national provisions
has been treated with biocide products (this then concerns a
apply.
treated product as defined by the (EU) Ordinance on Biocide
Products No. 528/2012): no
Application
Gradus Premium Loop Pile Tufted, Bitumen Backed Carpet Tile Reference service life
with Nylon Face Fibre is suitable for use as a floor covering in
When properly installed as a commercial floor covering, Gradus
heavy and general commercial installations.
Premium Loop Pile Tufted, Bitumen Backed Carpet Tile with
Nylon face fibre has a reference service life of 12 years. This
Technical Data
carpet tile product comes with a 12-year warranty and 10-year
The technical specifications of the product are listed on the
antistatic warranty, subject only to installation and maintenance
product's specification sheet, found at www.gradus.com. This
being carried out in accordance with the manufacturer's
2 Environmental Product Declaration - Gradus Ltd. - Gradus Carpet Tile with Nylon Face Fibre
guidelines.
LCA: Calculation rules
• Module B4 - Replacement (module not relevant).
Declared Unit • Module B5 - Refurbishment (module not relevant).
The declaration refers to the declared unit of 1 m² of installed • Module B6 - Operational Energy Use (module not
carpet tile. relevant).
Declared unit • Module B7 - Operational Water Use (module not
relevant).
Name Value Unit
End of Life Stage:
Declared unit 1 m2 Three scenarios have been evaluated:
Grammage 3.896 kg/m2 Scenario 1: the Gradus Bitumen Backed carpet is 100%
Layer thickness 0.006 m disposed of in a landfill.
Scenario 2: the Gradus Bitumen Backed carpet is 100%
incinerated.
System boundary
Scenario 3: 40% of Gradus Bitumen Backed carpets are
The type of EPD is Cradle-to-Gate with options modules C1–
incinerated and the remaining 60% are landfilled. This
C4, module D, and additional modules. The additional modules
assumption is based on the carpet disposal rates in Europe
are A4, A5, B1 and B2.
mentioned in the study conducted by Deutsche Umwelthilfe in
2017 (Umwelthilfe, 2017) and the European Commission in
The modules considered in the life cycle assessment and
2013 (Commission, 2013).
environmental product declaration, based on the product's
entire life cycle, are described as follows: • Module C1 - The carpet is de-constructed manually and
no additional environmental impact is caused.
Production Stage: • Module C2 - Transport of the carpet waste to a landfill or
to the municipal waste incineration plant.
• Module A1 - Provision of Raw Materials.
• Module C3 - Impacts from thermal treatment disposal
• Module A2 - Transport of Raw Materials.
(C3/2 and C3/3).
• Module A3 - Manufacturing.
• Module C4 - Impacts from landfill disposal (C4/1 and
Construction/Installation Stage:
C4/3).
• Module A4 - Transportation by truck of the product to the Module D includes benefits from energy recovery via treatment
construction site in Europe. of packaging materials and incineration of carpets at their end
• Module A5 - Installation of the carpet, treatment of of life (D/1, D/2 and D/3), as well as the burdens of balancing
cutting waste (landfill) and packaging waste (landfill, the secondary material content in modules A1 and A3 via the
recycling, and incineration). The production of the net-scrap approach.
amount of carpet that occurs as installation waste is
also included along with its transport to the place of Geographic Representativeness
installation. Biogenic carbon that is stored in the wooden Land or region, in which the declared product system is
pallets and cardboard (packaging) is released as carbon manufactured, used or handled at the end of the product´s
dioxide emissions into the air at the end of life in module lifespan: Europe
A5.
Use Stage:
Comparability
• Module B1 - Indoor emissions of volatile organic
Basically, a comparison or an evaluation of EPD data is only
compounds (VOCs) during the first few months after
possible if all the data sets to be compared were created
installation.
according to EN 15804 and the building context, respectively
• Module B2 - Carpet cleaning per year, including
the product-specific characteristics of performance, are taken
vacuuming (electricity consumption) and hot water
into account. The background database used for the creation of
cleaning (electricity and water consumption, as well as
the EPD: GaBi ts software, CUP 2022.2.
waste water treatment).
• Module B3 - Repair (module not relevant).
LCA: Scenarios and additional technical information
Name Value Unit
Characteristic product properties of biogenic carbon
Transport distance (truck) 687 km
Biogenic carbon is only present in packaging (wooden pallets
Capacity utilisation (including empty runs) 55 %
and cardboards). Assumed water content in wooden pallet
(packaging): 18%.
Installation in the building (A5)
Information on describing the Biogenic Carbon Content at The installation of Gradus Bitumen Backed Carpet Tile is done
factory gate manually and no energy is required. A Pressure-Sensitive
Name ValueUnit adhesive is required for the installation of Gradus Bitumen
Biogenic carbon content in accompanying kg Backed Carpet Tile and should be used in accordance with the
packaging 0.14 C manufacturer's guidelines. Installation losses have been
accounted for in module A5. Product losses are considered as
5%.
The following technical scenario information is required for the
declared modules and optional for non-declared modules.
The packaging material treatment and disposal are also
Transport to the construction site (A4) considered in module A5 (landfill, recycling, and incineration)
3 Environmental Product Declaration - Gradus Ltd. - Gradus Carpet Tile with Nylon Face Fibre
and the resulting benefits from energy generation are included
End of Life (C1-C4)
in module D. The quantity of wooden pallets used is 0.133 kg
C1 - The product dismantling from the building is done
per m². Wooden pallets are assumed to be re-used 20 times
manually without energy burden.
before being disposed of. Hence, the quantity of pallet disposed
C2 - Transportation of the product to the end of life is assumed
is 0.007 kg. The quantity of cardboard packaging is 0.21 kg/m²
to be 161 km (100 miles).
and the quantity of plastic packaging is 0.0103 kg/m². Total
C3/2 - The Gradus Bitumen Backed carpet is 100% combusted
amount of packaging disposed at installation is 0.227 kg.
in an incineration plant with energy recovery (R>0.6).
Packaging disposal rates (Source: Eurostat, Recovery and
C3/3 - It is assumed that 40% of Gradus Bitumen Backed
recycling rates for packaging).
carpets are incinerated and the remaining 60% are landfilled.
• Paper - 82.8% recycled; 9.4% landfilled; and 7.8% C4/1 - The Gradus Bitumen Backed carpet is 100% disposed of
incinerated in landfill.
• Plastic - 40.3% recycled; 28.7% landfilled; and 31.0% C4/3 - It is assumed that 40% of Gradus Bitumen Backed
incinerated carpets are incinerated and the remaining 60% are landfilled.
• Wood pallets - 39.8% recycled; 34.5% landfilled; and
Name ValueUnit
25.7% incinerated
Collected as mixed construction waste 3.896 kg
Name ValueUnit
Landfilling (Scenario 1 - C3/1, C4/1 and D/1) 3.896 kg
Auxiliary 0.23 kg
Incineration (Scenario 2 - C3/2, C4/2, and D/2) 3.896 kg
Material loss 0.203 kg
Landfilling (60%) and Incineration (40%) (Scenario
Output substances following waste treatment on 3.896 kg
0.227 kg 3 - C3/3, C4/3 and D/3)
site (packaging materials)
Maintenance (B2) Reuse, recovery and/or recycling potentials (D), relevant
For the maintenance of Gradus Bitumen Backed Carpet Tile, 2 scenario information
hot water extraction cleanings (water and electricity For the thermal and electrical energy generated in Module A5
consumption) per year as well as 52 vacuum cleanings due to thermal treatment of packaging, avoided burdens have
(electricity consumption) per year are recommended. The been calculated by the inversion of electricity grid mix and
Reference Service Life of the product is 12 years. The results in thermal energy from natural gas, using European datasets.
the EPD declare a maintenance for the period of 1 year. Module D also includes the environmental burdens linked to the
Name Value Unit supply to secondary materials (nylon and calcium carbonate)
used in the carpet production.
Water consumption (1 year) 0.0009 m3
Electricity consumption (1 year) 0.772 kWh
Reference service life
Name ValueUnit
Reference service life (according to ISO 15686-1, -
12 a
2, -7 and -8)
Life Span according to the manufacturer 12 a
4 Environmental Product Declaration - Gradus Ltd. - Gradus Carpet Tile with Nylon Face Fibre
LCA: Results
The B2 module declares the maintenance (cleaning) per one year. The user of the EPD will be able to scale the results for its entire
useful life by multiplying the impact by the RSL.
The LCA results presented below applies to 100% landfilled end of life scenario.
DESCRIPTION OF THE SYSTEM BOUNDARY (X = INCLUDED IN LCA; MND = MODULE OR INDICATOR NOT DECLARED; MNR
= MODULE NOT RELEVANT)
Benefits and
Construction loads beyond
Product stage Use stage End of life stage
process stage the system
boundaries
la ire ta m w a Ry lp p u s tro p s n a rT g n iru tc a fu n a M e h t m o rf tro p s n a rTe tis e h t o t e ta g y lb m e s s A e s U e c n a n e tn ia M ria p e R tn e m e c a lp e R tn e m h s ib ru fe R y g re n e la n o ita re p Oe s u re ta w la n o ita re p Oe s u n o itc u rts n o c -e Dn o itilo m e d tro p s n a rT g n is s e c o rp e ts a W la s o p s iD -e s u e R-y re v o c e R-g n ilc y c e Rla itn e to p
A1 A2 A3 A4 A5 B1 B2 B3 B4 B5 B6 B7 C1 C2 C3 C4 D
X X X X X X X MNR MNR MNR MND MND X X X X X
RESULTS OF THE LCA - ENVIRONMENTAL IMPACT according to EN 15804+A2: 1 m² Gradus Bitumen Backed Carpet
Parameter Unit A1-A3 A4 A5 B1 B2 C1 C2 C3 C4 D
GWP-total kg CO 2 eq 7.58E+00 2.45E-01 5.05E-01 2.54E-04 2.32E-01 0 5.28E-02 0 2.73E-01 -1.72E-02
GWP-fossil kg CO 2 eq 7.9E+00 2.44E-01 5.08E-01 2.54E-04 2.29E-01 0 5.26E-02 0 2.76E-01 -2.11E-02
GWP-
biogenic kg CO 2 eq -3.28E-01 -3.37E-04 -3.64E-03 0 2.44E-03 0 -7.26E-05 0 -2.94E-03 3.88E-03
GWP-luluc kg CO 2 eq 3.38E-03 1.36E-03 2.87E-04 0 4.85E-05 0 2.93E-04 0 1.34E-04 -3.19E-06
ODP kg CFC11 eq 8.28E-09 1.46E-14 4.36E-10 0 3.35E-12 0 3.15E-15 0 3.71E-13 -1.22E-13
AP mol H+ eq 1.43E-02 2.51E-04 1.17E-03 0 5.03E-04 0 5.42E-05 0 8.18E-04 -3.47E-05
EP-
kg P eq 2.07E-05 7.28E-07 1.57E-05 0 1.12E-06 0 1.57E-07 0 5.15E-05 -3.08E-08
freshwater
EP-marine kg N eq 3.63E-03 8.22E-05 2.66E-04 0 1.15E-04 0 1.77E-05 0 1.81E-04 -9.64E-06
EP-terrestrial mol N eq 3.46E-02 9.79E-04 3.27E-03 0 1.18E-03 0 2.11E-04 0 1.99E-03 -1.03E-04
kg NMVOC
POCP 1.22E-02 2.21E-04 9.72E-04 1.41E-05 3.05E-04 0 4.77E-05 0 5.83E-04 -3.14E-05
eq
ADPE kg Sb eq 1.04E-06 2.04E-08 7.99E-08 0 6.24E-08 0 4.4E-09 0 1.92E-08 -3.33E-09
ADPF MJ 1.73E+02 3.26E+00 1.05E+01 0 4.15E+00 0 7.03E-01 0 3.92E+00 -5.01E-01
m3 world eq
WDP 3.57E-01 2.19E-03 8.86E-02 0 5.23E-02 0 4.72E-04 0 -2.72E-03 -2.98E-03
deprived
GWP = Global warming potential; ODP = Depletion potential of the stratospheric ozone layer; AP = Acidification potential of land and water; EP =
Eutrophication potential; POCP = Formation potential of tropospheric ozone photochemical oxidants; ADPE = Abiotic depletion potential for non-fossil
resources; ADPF = Abiotic depletion potential for fossil resources; WDP = Water (user) deprivation potential)
RESULTS OF THE LCA - INDICATORS TO DESCRIBE RESOURCE USE according to EN 15804+A2: 1 m² Gradus Bitumen
Backed Carpet
Parameter Unit A1-A3 A4 A5 B1 B2 C1 C2 C3 C4 D
PERE MJ 1.21E+01 1.95E-01 5.11E+00 0 2.31E+00 0 3.99E-02 0 3.22E-01 -1.29E-01
PERM MJ 5.31E+00 0 -4.19E+00 0 0 0 0 0 0 0
PERT MJ 1.74E+01 1.95E-01 9.21E-01 0 2.31E+00 0 3.99E-02 0 3.22E-01 -1.29E-01
PENRE MJ 1.31E+02 3.44E+00 1.57E+00 0 4.15E+00 0 7.04E-01 0 3.92E+00 -5.02E-01
PENRM MJ 5.1E+01 0 -3.17E-01 0 0 0 0 0 0 0
PENRT MJ 1.81E+02 3.44E+00 1.26E+00 0 4.15E+00 0 7.04E-01 0 3.92E+00 -5.02E-01
SM kg 1.1E-01 0 5.77E-03 0 0 0 0 0 0 -1.15E-01
RSF MJ 0 0 0 0 0 0 0 0 0 0
NRSF MJ 0 0 0 0 0 0 0 0 0 0
FW m3 2.36E-02 2.1E-04 9.32E-03 0 2.2E-03 0 4.52E-05 0 5.07E-05 -1.05E-04
PERE = Use of renewable primary energy excluding renewable primary energy resources used as raw materials; PERM = Use of renewable primary
energy resources used as raw materials; PERT = Total use of renewable primary energy resources; PENRE = Use of non-renewable primary energy
excluding non-renewable primary energy resources used as raw materials; PENRM = Use of non-renewable primary energy resources used as raw
materials; PENRT = Total use of non-renewable primary energy resources; SM = Use of secondary material; RSF = Use of renewable secondary fuels;
NRSF = Use of non-renewable secondary fuels; FW = Use of net fresh water
RESULTS OF THE LCA – WASTE CATEGORIES AND OUTPUT FLOWS according to EN 15804+A2:
1 m² Gradus Bitumen Backed Carpet
Parameter Unit A1-A3 A4 A5 B1 B2 C1 C2 C3 C4 D
HWD kg 3.92E-07 1.56E-11 2.31E-08 0 3.59E-10 0 3.37E-12 0 6.04E-10 -4.49E-11
NHWD kg 2.94E-01 4.68E-04 2.48E-01 0 3.82E-03 0 1.01E-04 0 3.88E+00 -2.01E-04
RWD kg 3.52E-03 4.02E-06 2.05E-04 0 6.64E-04 0 8.67E-07 0 4.81E-05 -2.33E-05
5 Environmental Product Declaration - Gradus Ltd. - Gradus Carpet Tile with Nylon Face Fibre
CRU kg 0 0 0 0 0 0 0 0 0 0
MFR kg 0 0 1.81E-01 0 0 0 0 0 0 0
MER kg 0 0 0 0 0 0 0 0 0 0
EEE MJ 0 0 6.37E-02 0 0 0 0 0 0 0
EET MJ 0 0 9.77E-02 0 0 0 0 0 0 0
HWD = Hazardous waste disposed; NHWD = Non-hazardous waste disposed; RWD = Radioactive waste disposed; CRU = Components for re-use;
MFR = Materials for recycling; MER = Materials for energy recovery; EEE = Exported electrical energy; EET = Exported thermal energy
RESULTS OF THE LCA – additional impact categories according to EN 15804+A2-optional:
1 m² Gradus Bitumen Backed Carpet
Parameter Unit A1-A3 A4 A5 B1 B2 C1 C2 C3 C4 D
Disease
PM 1.36E-07 1.45E-09 1.2E-08 0 4.17E-09 0 3.13E-10 0 7.87E-09 -7.87E-10
incidence
IR kBq U235 eq 3.76E-01 5.9E-04 2.24E-02 0 1.12E-01 0 1.27E-04 0 7.11E-03 -3.92E-03
ETP-fw CTUe 9.28E+01 2.26E+00 5.93E+00 1.15E-04 1.88E+00 0 4.88E-01 0 3.83E+00 -1.94E-01
HTP-c CTUh 2.64E-09 4.56E-11 1.76E-10 0 5.43E-11 0 9.83E-12 0 1.72E-10 -5.75E-12
HTP-nc CTUh 1.34E-07 2.37E-09 9.28E-09 3.07E-12 2.12E-09 0 5.1E-10 0 1.44E-08 -2.24E-10
SQP SQP 1.4E+01 1.12E+00 1.12E+01 0 1.5E+00 0 2.42E-01 0 2.82E-01 -6.47E-01
PM = Potential incidence of disease due to PM emissions; IR = Potential Human exposure efficiency relative to U235; ETP-fw = Potential comparative
Toxic Unit for ecosystems; HTP-c = Potential comparative Toxic Unit for humans (cancerogenic); HTP-nc = Potential comparative Toxic Unit for humans
(not cancerogenic); SQP = Potential soil quality index
Disclaimer 1: For the indicator 'Potential Human exposure efficiency relative to U235". This impact category deals mainly with the
eventual impact of low dose ionizing radiation on human health of the nuclear fuel cycle. It does not consider effects due to possible
nuclear accidents, occupational exposure nor due to radioactive waste disposal in underground facilities. Potential ionizing radiation
from the soil, from radon and from some construction materials is also not measured by this indicator.
Disclaimer 2: For the indicators 'Abiotic depletion potential for non-fossil resources', 'Abiotic depletion potential for fossil resources”,
“Water (user) deprivation potential", "Deprivation-weighted water consumption”, “Potential comparative toxic unit for ecosystems”,
“Potential comparative toxic unit for humans -cancerogenic”, “Potential comparative toxic unit for humans -non-carcinogenic”, “Potential
soil quality index”. The results of these environmental impact indicators shall be used with care as the uncertainties on these results are
high or as there is limited experienced with the indicators. This EPD was created using a software tool.
References
STANDARDS: ISO 15686-2:2011, Building and constructed assets — Service
life planning — Part 2: Service life prediction procedures.
EN 10874
EN 10874:2009, Resilient, textile and laminate floor coverings ISO 15686
— Classification. ISO 15686-7:2011, Building and constructed assets — Service
life planning — Part 7: Performance evaluation for feedback of
EN 1307 service life data from practice.
EN 1307:2014, Textile floor coverings — Classification.
ISO 15686
EN 14041 ISO 15686-8:2011, Building and constructed assets — Service
EN 14041:2004/AC:2006 — Resilient, textile and laminate floor life planning — Part 8: Reference service life and service life
coverings — Essential characteristics. estimation.
EN 15804 FURTHER REFERENCES:
EN 15804:2012+A2:2019/AC:2021, Sustainability of
construction works — Environmental product declarations — Candidate list
Core rules for the product category of construction products. Candidate List of substances of very high concern for
Authorisation, published on ECHA website, latest version
ISO 14025 17.01.2023 (https://echa.europa.eu/candidatelist-table).
ISO 14025:2011, Environmental labels and declarations —
Type III environmental declarations — Principles and Deutsche Umwelthilfe
procedures. Deutsche Umwelthilfe. Swept under the Carpet: The Big Waste
Problem of the Carpet Industry in Germany, 2017.
ISO 14040
ISO 14040:2006, Environmental management — Life cycle Envision LCA Tool
assessment — Principles and framework. Envision LCA Tool, 2021, Sphera Solutions GmbH, Leinfelden-
Echterdingen, with acknowledgement of LBP University of
ISO 14044 Stuttgart, version 1.
ISO 14044:2006, Environmental management — Life cycle
assessment — Requirements and guidelines. GaBi
GaBi Software System and Database for Life Cycle
ISO 15686 Engineering, 1992-2021, Sphera Solutions GmbH, Leinfelden-
ISO 15686-1:2011, Building and constructed assets — Service Echterdingen, with acknowledgement of LBP University of
life planning — Part 1: General principles and framework. Stuttgart, program version GaBi 10; database version 2021.1.
ISO 15686 GaBi documentation
6 Environmental Product Declaration - Gradus Ltd. - Gradus Carpet Tile with Nylon Face Fibre
GaBi dataset documentation for the software system and Umwelt e.V., 2021.
databases, LBP, University of Stuttgart and Sphera Solutions
GmbH, Leinfelden-Echterdingen, 2021 (http://www.gabi- PCR Part B
software.com/support/gabi/gabi-database-2021-lci- Product Category Rules for Building Products, Part B:
documentation/). Requirements on the EPD for floor coverings, version 1.7, 2022
(www.bau-umwelt.de).
IBU 2021
Institut Bauen und Umwelt e.V.: General Instructions for the Packaging disposal rates
EPD programme of Institut Bauen und Umwelt e.V., Version Eurostat, Recovery and recycling rates for packaging. 2015
2.0, Berlin: Institut Bauen und Umwelt e.V., 2021 (www.ibu- (http://ec.europa.eu/eurostat/web/environment/waste/main-
epd.com). tables).
The literature referred to in the Environmental Product
PCR Part A Declaration must be listed in full.Standards already fully quoted
PCR Part A: Calculation rules for the Life Cycle Assessment in the EPD do not need to be listed here again.
and Requirements on the Background Report according to EN The current version of PCR Part A and PCR Part B of the PCR
15804:2012+A2:2019/AC:2021, Version 1.3, Institut Bauen und document on which they are based must be referenced.
7 Environmental Product Declaration - Gradus Ltd. - Gradus Carpet Tile with Nylon Face Fibre
Publisher
Institut Bauen und Umwelt e.V. +49 (0)30 3087748- 0
Hegelplatz 1 info@ibu-epd.com
10117 Berlin www.ibu-epd.com
Germany
Programme holder
Institut Bauen und Umwelt e.V. +49 (0)30 3087748- 0
Hegelplatz 1 info@ibu-epd.com
10117 Berlin www.ibu-epd.com
Germany
Author of the Life Cycle Assessment
Sphera Solutions GmbH +49 711 341817-0
Hauptstraße 111- 113 info@sphera.com
70771 Leinfelden-Echterdingen www.sphera.com
Germany
Owner of the Declaration
Gradus Ltd. +44 0 1625428922
Chapel Mill, Park Green * imail@gradus.com
SK11 7LZ Mecclesfield, Cheshire www.gradus.com
United Kingdom
8 Environmental Product Declaration - Gradus Ltd. - Gradus Carpet Tile with Nylon Face Fibre
