ENVIRONMENTAL PRODUCT DECLARATION
as per ISO 14025 and EN 15804+A2
Owner of the Declaration KE Fibertec AS
Publisher Institut Bauen und Umwelt e.V. (IBU)
Programme holder Institut Bauen und Umwelt e.V. (IBU)
Declaration number EPD-KEF-20230265-CBI1-EN
Issue date 21.12.2023
Valid to 20.12.2028
GreenWeave textile-based ventilation duct
KE Fibertec AS
www.ibu-epd.com | https://epd-online.com
General Information
KE Fibertec AS GreenWeave textile-based ventilation duct
Programme holder Owner of the declaration
IBU – Institut Bauen und Umwelt e.V. KE Fibertec AS
Hegelplatz 1 Industrivej Vest 21
10117 Berlin 6600 Vejen
Germany Denmark
Declaration number Declared product / declared unit
EPD-KEF-20230265-CBI1-EN 1 kg of GreenWeave ventilation duct including mounting equipment.
This declaration is based on the product category rules: Scope:
Ventilation ducts, 01.08.2021 This is a representative EPD describing the production of 1 kg KE Fibertec
(PCR checked and approved by the SVR) AS custom-made textile-based ventilation ducts of the GreenWeave (GW)
line including mounting equipment. KE Fibertec AS have two production
sites. One in Vejen in Denmark, which includes both a weaving mill, laser
Issue date cutting and sewing room. The other production site is located in the Czech
Republic and includes laser cutting and a sewing room. Both sites are
21.12.2023
included in the results of this EPD.
The main component of the textile duct is polyester and the mounting
Valid to
equipment is made of aluminium. The data represents the production of
20.12.2028 2021.
The owner of the declaration shall be liable for the underlying information
and evidence; the IBU shall not be liable with respect to manufacturer
information, life cycle assessment data and evidences.
The EPD was created according to the specifications of EN 15804+A2. In
the following, the standard will be simplified as EN 15804.
Verification
The standard EN 15804 serves as the core PCR
Independent verification of the declaration and data according to ISO
14025:2011
Dipl.-Ing. Hans Peters
(Chairman of Institut Bauen und Umwelt e.V.) internally X externally
Florian Pronold Ms Jane Anderson,
(Managing Director Institut Bauen und Umwelt e.V.) (Independent verifier)
1 Environmental Product Declaration - KE Fibertec AS - GreenWeave textile-based ventilation duct
Product
Aluminium rail:
Product description/Product definition
• BS EN 573-3:2019+A1
This is a representative EPD representing the GreenWeave
• EN 515
product group. The textile ducts made by KE Fibertec A/S are
• DIN EN 10204 2.2
either round, semi-round or quarter-round ducts made of a light
weight textile material. They are designed for delivery and Technical data
distribution of cooled or heated air. The textile is suitable for Name Value Unit
ventilation purposes in schools, offices, shops, showrooms
Material textile duct Polyester -
production facilities and food industry, and other types of
Material used for mounting Aluminium -
rooms. The textile ducts primarily consist of two parts. One
Meter weight Duct incl. mounting material 1 - 3 kg/m
being the textile tube and the other the mounting equipment
consisting of an aluminium rail. The textile used is Operating Temperature (max. permitted) 80 °C
manufactured at KE Fibertec's own weaving mill and is Operating Temperature (min. permitted) -45 °C
designed for air distribution. The mounting equipment is made
Performance data of the product with respect to its
of aluminium. Textile ducts can be equipped with nozzles to
characteristics in accordance with the relevant technical
enhance good ventilation in large rooms.
provision (no CE-marking).
The production of KE Fibertec's textile-based ventilation ducts
have so far not been subject to EU harmonisation legislation. Base materials/Ancillary materials
Hence, for the use and application of the products the
Name Value Unit
respective national provisions at the place of use apply.
Textile Polyester 37 %
Application Aluminium Mounting equipment 54 %
KE Fibertecs GreenWeave textile-based ventilations ducts are Ancillary materials 9 %
custom-made to provide the optimal service in the specific room
This product/article/at least one partial article contains
and under the specific conditions they are placed in. The
substances listed in the candidate list (date: 15.05.2023)
ventilation ducts are made for blowing in and distributing air.
exceeding 0.1 percentage by mass: No
Technical Data
Reference service life
The main components - polyester and aluminium - of the
No reference service life is declared since the complete use
ventilation duct covered by this EPD are tested in accordance
stage is not included. However, the expected life-time of the
with the following standards.
product is estimated to be 25 years. Some of the ventilation
Polyester:
ducts are over 35 years and still in service. The life-time of the
• ISO 9001
product depends on the operation conditions and maintenance
• EN 779
of the product.
• DS 428
• EN 13501-1
LCA: Calculation rules
Declared unit
Declared Unit
The declared unit is 1 kg of GreenWeave ventilation duct Name Value Unit
including mounting equipment. This study describes the Declared unit 1 kg
environmental impacts of a representative textile-based Mass reference 1 - 3 kg/rm
ventilation duct of the GreenWeave line manufactured at KE
Raw density Polyester 500 kg/m3
Fibertec. The input material represents a weighted average for
all the products under the given product group. The data is This is a representative EPD representing an average
based on the production in 2021 and the total production GreenWeave ventilation duct as these are always costum
volume of the same period. The processing at the production made. The representative product is compiles based on 5
site is almost identical for the different products. The only cases. The main components of the ventilation duct are the
difference is the amount of clipping and the addition of nozzles aluminium rail for mounting and the polyester. The smaller the
for one type of ventilation duct. An average amount of clippings ducts (length and diameter) the higher the share of aluminium.
is applied in this study and an amount of nozzle is added in the The standard variation within the aluminium and polyester input
modelling. is 4 and 5 %, respectively. This means that the environmental
This EPD represents the GreenWeave product group. The impact of smaller ventilation ducts where the share of
differences within the GreenWeave ventilation ducts are the aluminium is higher the environmental impact will be higher
dimensions and permeability of the fabric. However, the compared to larger ventilation ducts where the share of
production processes of the products within the GreenWeave aluminium will be smaller.
line are the same. Therefore, a representative EPD is made to
System boundary
cover this product group. The representative product is
compiled by using 5 solutions varying in size and calculating a This is a cradle-to-gate EPD - with options, including the
weighted average of each component of the ventilation duct. modules A1-A3, B2, C1-4 and D.
Production stage - Modules A1-3
The production stage includes:
• A1, raw material extraction and processing, processing
of secondary material from previous product systems,
2 Environmental Product Declaration - KE Fibertec AS - GreenWeave textile-based ventilation duct
when applicable. KE Fibertec have due to their cradle-to-cradle certification focus
• A2, transport to factory gate and internal transport on recyclability of their produkt. KE Fibertec has established a
• A3, manufacturing of products and packaging, as well takeback scheme to increase the amount of recycled material in
as assembly and processing up to the end-of-waste their products. Hence, most of the material is send to recycling
state. within their take back scheme. The waste processes in C3
All of the above-mentioned are included in this study. Wastes include the sorting of aluminium, polyester, POM, nylon, and
and losses of the manufacturing processes are included in the steel. The following sorting efficiencies have been used:
processes in which they occur according to the polluter pays
principle. The construction of the manufacturing facility is not Aluminium - 98 % recycling and 2 % landfill
taken into account. Polyester - 91.3 % recycling and 8.7 % incineration with energy
recovery
For the environmental impact, the use of green electricity was POM - 90.5 % recycling and 9.5 % incineration with energy
calculated taking into account the residual electricity mix for the recovery
remaining electricity. The proportion of the electricity demand Steel - 96 % recycling and 4 % landfill
covered by green electricity in the total electricity demand in A3 Other - 100 % recycling
is 90%.
C3 also includes the incineration of the above mentioned
Use stage - Module B2 maintenance materials as well as regranulation of the polyester. After this all
The use stage includes: the material have entered the end-of-waste stage.
B2, maintenanceThe permeability of the textile ducts will
decrease over time due to depositions of dust and particles. Benefits and loads beyond the system boundaries -
Therefore, the ducts need to be washed regularly. KE Fibertec Module D
provides a washing service for their customers. The customer The benefits and loads include:
sends the ducts to KE Fibertec, who will then wash the ducts
• D, potential benefits from reuse, recycling and recovery
and deliver them back to the customer. The washing service
outside the scope of the study
included in this study includes transport, the use of water,
• D, potential loads related to processing to reach
electricity, detergent as well as the washing machine itself. The
equivalent materials to virgin input material
transport distance is not known and was assumed to be 300
In this EPD, the recycling of the main components - fabric and
km. The 300 km from the production site in Vejen in Denmark
aluminium is credited. Credit is only given to the net production
will cover the entire territory of Denmark. The washing service
of primary material. Steel and polyoxymethylene (POM) from
is primarily used by customers located relatively close to Vejen
small mounting materials and nozzles are also credited in this
as the service should be viable. A sensitivity test was made for
module. Also, here the amount of secondary material is
the transport distance by changing the distance to 600 km and
considered, and credit is only given to the avoidance of primary
the result showed, that it did not change the overall conclusion.
material. As described above module D includes the loads and
B2 is calculated based on 1 washing cycle. The amount of
benefits beyond system boundaries. To account for the loads
cycles during the lifetime of the ventilation duct varies between
required to achieve functional equivalence to the input material
application type. They are maximum washed 2 times every year
the processing of remelting aluminium and processing of fabric
and minimum once every 10 years. On average the ventilation
is accounted for. The same applies to the small fractions of
ducts are washed 1 time per year.
steel. Since a small fraction of plastic products such as
This EPD entails 2 B2 scenarios. B2 and B2/1.
polyester and nylon is incinerated heat and electricity are
B2 is a reference scenario using a European electricity mixB2/1
recovered and a credit for this is given in this module.
is using Danish wind power representing the washingservice
provided by KE Fibertec. Geographic Representativeness
Land or region, in which the declared product system is
End-of-life stage - Modules C1-C4 manufactured, used or handled at the end of the product´s
The end-of-life stage includes: lifespan: Denmark
C1, deconstruction and demolition
C2, transport to waste processing
C3, waste processing for reuse, recovery and/or recycling Comparability
C4, disposalThe deconstruction of the products is assumed to Basically, a comparison or an evaluation of EPD data is only
be done manually. As a result, no processes have been added possible if all the data sets to be compared were created
to module C1. The ventilation ducts are sold on the global according to EN 15804 and the building context, respectively
market. This means that transportation distance, technology the product-specific characteristics of performance, are taken
and waste processing are modelled accordingly. End-of-life into account. The system model EN15804 - cut-off available in
treatment of packaging material is not included as module A5 is the LCI database Ecoinvent v. 3.9 is used in this EPD
not declared.
LCA: Scenarios and additional technical information
Name ValueUnit
Characteristic product properties of biogenic carbon
kg
The biogenic carbon content quantifies the amount of biogenic Biogenic carbon content in product -
C
carbon in a construction product leaving the factory gate. Both
Biogenic carbon content in accompanying kg
the biogenic content of the product and the accompanying 0.035
packaging Cardboard C
packaging are declared.
Note: 1 kg of biogenic carbon is equivalent to 44/12 kg of CO 2. The following technical scenario information can be used for
the declared modules and optional modules for non-declared
Information on describing the biogenic carbon content at
modules. The following technical scenario information covers
factory gate
the disposal of the accompanying packaging material,
3 Environmental Product Declaration - KE Fibertec AS - GreenWeave textile-based ventilation duct
produced in module A3, on the construction site as module A5
Reuse, recovery and/or recycling potentials (D), relevant
is not declared in this EPD, B2 maintenance, end-of-life and
scenario information
loads and benefits beyond the system boundaries.
The following values in the table are amounts contributing to
Assembly (A5) the loads and benefits included in module D.
Name Value Unit Name Value Unit
Cardboard Packaging waste for recycling 0.07 kg Recycling of polyester From module C3 0.36 kg
Recycling of aluminium From module C3 0.14 kg
Maintenance (B2)
Recycling of POM From module C3 0.03 kg
This module includes the washing service of KE Fibertec. A
sensitivity analysis was made on the transportation distance Recycling of steel From module C3 0.0004 kg
and showed that doublling the distance does not change the Incineration of polyester From module C3 0.02 kg
overall conclusion of the EPD. Module B2 represents 1 the Incineration of POM From module C3 0.002 kg
input for 1 washing cycle and a ventilation ducts is an average
Incineration of other material From module C3 0.01 kg
washed once a year.
Two scenarios are made for the washing service. One using Credits are only given to the net amount leaving the product
European power mix as describes in PCR part 1 (B2/1) and one system that has passed the end-of-waste state. In the LCA
representing KE Fibertec washing service at their facilities in calculation loads related to obtaining equivalent functions as
Denmark. For the second scenario at KE Fibertecs facility the original virgin material are included as well as the benefits
transport is included (B2/2). of avoided production of the given virgin material.
Name Value Unit
Expected life-time 25 years
Maintenance cycle 26 Number/RSL
Water consumption per cycle 0.24 m3
Detergent per cycle 0.05 L
Washing load per cycle 12 kg
Electricity consumption per cycle 0.15 kWh
Transport distance 300 km
End of life (C1-C4)
The following table shows the technical information scenario
regarding waste module C stating the different waste fractions
and their collection form and waste processing steps. The
transportation distances have been assumed as no data on
average distances to waste treatment facilities have been
found. However, a sensitivity analysis was conducted doubling
the transportation distances. The test showed, that changing
the distances did not have a significant influence on the overall
results and did not change the overall conclusion.
KE Fibertec has established a takeback scheme, hence a large
part of the products are recycled. This has been done as a part
of KE Fibertecs Cradle-to-cradle certifikation.
Name Value Unit
Collected separately waste type 1 kg
Polyester 0.40 kg
Aluminium 0.54 kg
POM 0.03 kg
Steel 0.02 kg
Other material 0.01 kg
Recycling Polyester 0.36 kg
Recycling Aluminium 0.53 kg
Recycling POM 0.03 kg
Recycling Steel 0.02 kg
Energy recovery Polyester 0.04 kg
Energy recovery POM 0.002 kg
Energy recovery Other material 0.01 kg
Landfilling Aluminium 0.01 kg
Landfilling Steel 0.001 kg
Transport Sorting 200 km
Transport Recycling 100 km
Transport Incineration 100 km
Transport Landfil 150 km
4 Environmental Product Declaration - KE Fibertec AS - GreenWeave textile-based ventilation duct
LCA: Results
The following table shows the LCA results obtained in this study.
For calculation of the results, characterization was used on a model created of individual inputs from different LCIA methods to comply
with EN15804+A2 which is yet to be fully implemented in the SimaPro software. As a result, the LCIA has been calculated in Excel
using the following methods from EcoInvent v.3.9:
• EF v.3.1 EN 15804
• EN 15804 inventory indicators according to ISO 21930
The additional indicators are retrieved by using ecoinvent cumulative LCIA results for the system model EN15804, cut-off. It follows ISO
21930 for all the datasets; hence the results include all the background processes as well as foreground processes.
C1 is declared as 0 since manual deconstruction is assumed.
The estimated impact results are only relative statements which do not indicate the end-points of the impact categories, exceeding
threshold values, safety margins or risks.
DESCRIPTION OF THE SYSTEM BOUNDARY (X = INCLUDED IN LCA; MND = MODULE OR INDICATOR NOT DECLARED; MNR
= MODULE NOT RELEVANT)
Benefits and
Construction loads beyond
Product stage Use stage End of life stage
process stage the system
boundaries
la ire ta m w a Ry lp p u s tro p s n a rT g n iru tc a fu n a M e h t m o rf tro p s n a rTe tis e h t o t e ta g y lb m e s s A e s U e c n a n e tn ia M ria p e R tn e m e c a lp e R tn e m h s ib ru fe R y g re n e la n o ita re p Oe s u re ta w la n o ita re p Oe s u n o itc u rts n o c -e Dn o itilo m e d tro p s n a rT g n is s e c o rp e ts a W la s o p s iD -e s u e R-y re v o c e R-g n ilc y c e Rla itn e to p
A1 A2 A3 A4 A5 B1 B2 B3 B4 B5 B6 B7 C1 C2 C3 C4 D
X X X MND MND MND X MNR MNR MNR MND MND X X X X X
RESULTS OF THE LCA - ENVIRONMENTAL IMPACT according to EN 15804+A2: 1 kg GreenWeave ventilation duct incl.
mounting equipment
Parameter Unit A1-A3 B2 B2/1 C1 C2 C3 C4 D
GWP-total kg CO 2 eq 6.49E+00 8.49E-01 7.71E-01 0 1.48E-01 6.9E-01 1.82E-04 -2.26E+00
GWP-fossil kg CO 2 eq 6.46E+00 8.71E-01 7.93E-01 0 1.48E-01 5.86E-01 1.68E-04 -2.23E+00
GWP-biogenic kg CO 2 eq 1.78E-02 0 0 0 1.29E-04 1.04E-01 1.42E-05 -3.39E-03
GWP-luluc kg CO 2 eq 3.9E-02 5.34E-02 5.34E-02 0 7.3E-05 4.15E-04 5.02E-08 -2.49E-02
ODP kg CFC11 eq 7.71E-06 1.7E-08 1.54E-08 0 3.22E-09 1.23E-08 4.45E-12 -4.59E-06
AP mol H+ eq 3.5E-02 2.8E-03 2.39E-03 0 3.23E-04 1.36E-03 1.1E-06 -1.34E-02
EP-freshwater kg P eq 2.38E-03 1.32E-04 9.34E-05 0 1.05E-05 1.43E-04 2.03E-08 -6.96E-04
EP-marine kg N eq 7.42E-03 1.16E-03 1.09E-03 0 8.2E-05 1.04E-03 4.49E-07 -1.93E-03
EP-terrestrial mol N eq 6.88E-02 7.15E-03 6.49E-03 0 8.28E-04 3.8E-03 4.9E-06 -1.96E-02
kg NMVOC
POCP 2.76E-02 3.34E-03 3.11E-03 0 5.01E-04 1.25E-03 1.73E-06 -7.43E-03
eq
ADPE kg Sb eq 7.42E-05 3.57E-06 3.52E-06 0 4.94E-07 2.4E-06 7.71E-10 2.29E-05
ADPF MJ 1.07E+02 1.37E+01 1.23E+01 0 2.11E+00 4.51E+00 3.56E-03 -3.93E+01
m3 world eq
WDP 6.08E+00 4.77E-01 4.61E-01 0 1.05E-02 1.13E-01 9.1E-05 -1.96E+00
deprived
GWP = Global warming potential; ODP = Depletion potential of the stratospheric ozone layer; AP = Acidification potential of land and water; EP =
Eutrophication potential; POCP = Formation potential of tropospheric ozone photochemical oxidants; ADPE = Abiotic depletion potential for non-fossil
resources; ADPF = Abiotic depletion potential for fossil resources; WDP = Water (user) deprivation potential)
RESULTS OF THE LCA - INDICATORS TO DESCRIBE RESOURCE USE according to EN 15804+A2: 1 kg GreenWeave
ventilation duct incl. mounting equipment
Parameter Unit A1-A3 B2 B2/1 C1 C2 C3 C4 D
PERE MJ 2.03E+01 2.19E+00 2.19E+00 0 3.3E-02 6.81E-01 6.26E-04 -6.55E+00
PERM MJ 0 0 0 0 0 0 0 0
PERT MJ 2.03E+01 2.19E+00 2.19E+00 0 3.3E-02 6.81E-01 6.26E-04 -6.55E+00
PENRE MJ 9.03E+01 1.38E+01 1.38E+01 0 2.12E+00 2.12E+00 3.56E-03 -3.09E+01
PENRM MJ 8.26E+00 0 0 0 0 -8.16E+00 0 0
PENRT MJ 9.85E+01 1.38E+01 1.38E+01 0 2.12E+00 -6.04E+00 3.56E-03 -3.09E+01
SM kg 2.5E-01 0 0 0 0 0 0 6.26E-01
RSF MJ 0 0 0 0 0 0 0 0
NRSF MJ 0 0 0 0 0 0 0 0
FW m3 1.3E-01 3.31E-02 3.2E-02 0 2.55E-04 2.97E-03 4.87E-06 -3.78E-02
PERE = Use of renewable primary energy excluding renewable primary energy resources used as raw materials; PERM = Use of renewable primary
energy resources used as raw materials; PERT = Total use of renewable primary energy resources; PENRE = Use of non-renewable primary energy
excluding non-renewable primary energy resources used as raw materials; PENRM = Use of non-renewable primary energy resources used as raw
materials; PENRT = Total use of non-renewable primary energy resources; SM = Use of secondary material; RSF = Use of renewable secondary fuels;
5 Environmental Product Declaration - KE Fibertec AS - GreenWeave textile-based ventilation duct
NRSF = Use of non-renewable secondary fuels; FW = Use of net fresh water
RESULTS OF THE LCA – WASTE CATEGORIES AND OUTPUT FLOWS according to EN 15804+A2:
1 kg GreenWeave ventilation duct incl. mounting equipment
Parameter Unit A1-A3 B2 B2/1 C1 C2 C3 C4 D
HWD kg 3.72E-01 1.65E-02 1.21E-02 0 1.44E-03 1.25E-02 1.42E-04 -1.38E-01
NHWD kg 9.63E+00 5.64E-01 3.78E-01 0 4.37E-02 7.66E-01 1.19E-02 -3.12E+00
RWD kg 4.95E-05 3.18E-06 1.43E-06 0 1.69E-07 4.82E-06 1.3E-09 -1.27E-05
CRU kg 0 0 0 0 0 0 0 0
MFR kg 9.2E-02 0 0 0 0 8.76E-01 0 0
MER kg 9.28E-06 0 0 0 0 8.9E-02 0 0
EEE MJ 0 0 0 0 0 3.02E-01 0 0
EET MJ 0 0 0 0 0 5.29E-01 0 0
HWD = Hazardous waste disposed; NHWD = Non-hazardous waste disposed; RWD = Radioactive waste disposed; CRU = Components for re-use;
MFR = Materials for recycling; MER = Materials for energy recovery; EEE = Exported electrical energy; EET = Exported thermal energy
RESULTS OF THE LCA – additional impact categories according to EN 15804+A2-optional:
1 kg GreenWeave ventilation duct incl. mounting equipment
Parameter Unit A1-A3 B2 B2/1 C1 C2 C3 C4 D
Disease
PM 3.34E-07 6.05E-08 5.88E-08 0 1.1E-08 1.24E-07 2.43E-11 -1.47E-07
incidence
IR kBq U235 eq 7.85E-01 5.45E-02 2.3E-02 0 2.84E-03 8.33E-02 2.96E-05 -1.84E-01
ETP-fw CTUe 4.1E+01 9.82E+00 9.66E+00 0 1.03E+00 1.8E+00 8.88E-02 2.33E+00
HTP-c CTUh 9.01E-09 7.25E-10 6.86E-10 0 7.04E-11 6.72E-10 3.21E-13 -3.87E-09
HTP-nc CTUh 1.13E-07 9.99E-09 9.38E-09 0 1.5E-09 5.55E-09 2.83E-12 -3.55E-08
SQP SQP 2.3E+01 1.14E+01 1.11E+01 0 1.27E+00 2.02E+00 7.01E-03 -2.17E+00
PM = Potential incidence of disease due to PM emissions; IR = Potential Human exposure efficiency relative to U235; ETP-fw = Potential comparative
Toxic Unit for ecosystems; HTP-c = Potential comparative Toxic Unit for humans (cancerogenic); HTP-nc = Potential comparative Toxic Unit for humans
(not cancerogenic); SQP = Potential soil quality index
Disclaimer 1 – for the indicator 'Potential Human exposure efficiency relative to U235'. This impact category deals mainly with the
eventual impact of low-dose ionizing radiation on human health of the nuclear fuel cycle. It does not consider effects due to possible
nuclear accidents, occupational exposure or radioactive waste disposal in underground facilities. Potential ionizing radiation from the
soil, radon and from some construction materials is also not measured by this indicator.
Disclaimer 2 – for the indicators 'abiotic depletion potential for non-fossil resources', 'abiotic depletion potential for fossil resources',
'water (user) deprivation potential, deprivation-weighted water consumption', 'potential comparative toxic unit for ecosystems', 'potential
comparative toxic unit for humans – cancerogenic', 'Potential comparative toxic unit for humans - not cancerogenic', 'potential soil
quality index'. The results of this environmental impact indicator shall be used with care as the uncertainties on these results are high
as there is limited experience with the indicator.
References
Standards construction works — Environmental Product Declarations —
DIN EN 10204 2.2 Core rules for the product category of construction products.
DIN EN 10204 2.2, Metallic products - Types of inspection
documents (non-specific inspections) ISO 9001
ISO 9001:2015, Quality management systems – Requirements
DS 428
DS 428:2019, Fire protection of ventilation systems ISO 14025
EN ISO 14025:2011, Environmental labels and declarations —
EN 515 Type III environmental declarations — Principles and
EN 515:2017, Aluminium and aluminium alloys - Wrought procedures.
products - Temper designations
ISO 14040
BS EN 573-3:2019+A1 ISO 14040:2006, Environmental management –Life cycle
BS EN 573-3:2019+A1:2022, Aluminium and aluminium alloys. assessment - Principles and framework; English version
Chemical composition and form of wrought products Chemical
composition and form of products ISO 14044
ISO 14044:2006, Environment Management – Life Cycle
EN 779 Assessment – Requirements and Instructions; English version
EN 779:2012, Particulate air filters for general ventilation – EN ISO 14044:2006.
Determination of the filtration performance
ISO 21930
EN 13501-1 ISO 21930:2017, Sustainability in buildings and civil
EN 13501-1:2018, Fire classification of construction products engineering works — Core rules for environmental
and building elements – Part 1: Classification using data from product declarations of construction products and services
reaction to fire tests Fire class B-s1-d0
Further References
EN 15804 ECHA candidate list
EN 15804 EN 15804:2012+A2:2019+AC:2021, Sustainability of Candidate List of substances of very high concern for
6 Environmental Product Declaration - KE Fibertec AS - GreenWeave textile-based ventilation duct
Authorisation
https://echa.europa.eu/candidate-list-table [Accessed 25-05- IBU 2023
2023]. PCR Guidance-Text for Building-Related Products and
Services, Part B: Requirements on the EPD for Ventilation
EcoInvent 3.9 ducts, Version 1.0
EcoInvent database version 3.9, cut-off, EN15804model. LCIA
methodology EF v3.1 EN15804.Wernet, G., Baue,., Steubing, SimaPro 2023
B., Reinhard, J., Moreno-Ruiz, E., and Weidema, B., 2016. The LCA software SimaPro version 9.5.
ecoinvent database version 3 (part pp.1218–1230. [Accessed
25-05-2023]
IBU 2021
Product Category Rules for Building-Related Products
and Services, Part A: Calculation Rules for the Life
Cycle Assessment and Requirements on the Project
Report, Version 1.3
7 Environmental Product Declaration - KE Fibertec AS - GreenWeave textile-based ventilation duct
Publisher
Institut Bauen und Umwelt e.V. +49 (0)30 3087748- 0
Hegelplatz 1 info@ibu-epd.com
10117 Berlin www.ibu-epd.com
Germany
Programme holder
Institut Bauen und Umwelt e.V. +49 (0)30 3087748- 0
Hegelplatz 1 info@ibu-epd.com
10117 Berlin www.ibu-epd.com
Germany
Author of the Life Cycle Assessment
Viegand Maagøe +45 33349000
Nørre Farimagsgade 37 info@viegandmaagoe.dk
1364 København K viegandmaagoe.dk
Denmark
Owner of the Declaration
KE Fibertec AS +4575364200
Industrivej Vest 21 info@ke-fibertec.dk
6600 Vejen www.ke-fibertec.com/da/
Denmark
8 Environmental Product Declaration - KE Fibertec AS - GreenWeave textile-based ventilation duct
