ENVIRONMENTAL PRODUCT DECLARATION
as per ISO 14025 and EN 15804+A2
Owner of the Declaration Hansgrohe Group
Publisher Institut Bauen und Umwelt e.V. (IBU)
Programme holder Institut Bauen und Umwelt e.V. (IBU)
Declaration number EPD-HAN-20230021-ICC2-EN
Issue date 24.02.2023
Valid to 23.02.2028
Hand Showers
Hansgrohe Group
www.ibu-epd.com | https://epd-online.com
1. General Information
Hansgrohe Group Hand Showers
Programme holder Owner of the declaration
IBU – Institut Bauen und Umwelt e.V. Hansgrohe Group
Hegelplatz 1 Auestr. 5-9
10117 Berlin 77761 Schiltach
Germany Germany
Declaration number Declared product / declared unit
EPD-HAN-20230021-ICC2-EN One (1) piece of an average hand shower incl. packaging
This declaration is based on the product category rules: Scope:
Fittings and showers, 01.08.2021 This average EPD was determined on the basis of a weighted average of
(PCR checked and approved by the SVR) production volume from 2020 and relates to the plants in Wasselonne,
France, Offenburg and Schiltach, Germany and Alpharetta, USA. This
average EPD is valid for the whole product group of chrome plated hand
Issue date showers. The EPD was formed from >92% of the products involved in the
sales quantity.
24.02.2023
The owner of the declaration shall be liable for the underlying information
and evidence; the IBU shall not be liable with respect to manufacturer
information, life cycle assessment data and evidences.
Valid to
23.02.2028 The EPD was created according to the specifications of EN 15804+A2. In
the following, the standard will be simplified as EN 15804.
Verification
The standard EN 15804 serves as the core PCR
Independent verification of the declaration and data according to ISO
14025:2011
internally X externally
Dipl.-Ing. Hans Peters
(Chairman of Institut Bauen und Umwelt e.V.)
Florian Pronold Dr Naeem Adibi,
(Managing Director Institut Bauen und Umwelt e.V.) (Independent verifier)
1 Environmental Product Declaration - Hansgrohe Group - Hand Showers
2. Product
The hand showers are delivered singularly packaged. The
2.1 Product description/Product definition packaging is customized to the
Hand showers size of the product and supplies. Customers can order single
essentially comprise of a housing made of plastic materials or products or
metal and a jet multiple products with outer packaging. The products with the
disc as well as several assembly parts of various materials. The smallest and the largest volume have dimensions between
shower surface 55x52x264 mm and 200x90x300 mm.
is usually chrome-plated by means of various galvanic process
stages. 2.5 Base materials/Ancillary materials
The material composition (incl. packaging) of an average hand
For the use shower is as follows:
and application of the product the respective national provisions Name Value Unit
at the place
Cardboard, Paper 28.3 %
of use apply, in Germany for example the building codes of the
Acrylonitrile butadiene styrene 24.1 %
federal states
and the corresponding national specifications. Polyphenylene 18.5 %
Polybutylene terephthalate with GF 11.7 %
The products comply with Other Plastics 9.9 %
the applicable standards and regulations listed below. Following
Polypropylen with GF 5.0 %
standards apply to all hand showers and head showers to
Brass 1.2 %
prove product safety:
Other material 1.0 %
• EN 1112:2008: Sanitary tapware – Shower outlets for
Stainless steel 0.2 %
sanitary tapware for water supply systems of type 1 and
type 2 The parts which are made of brass contain between 0.2 and
• ISO 3822: Acoustics – Laboratory tests on noise 1.4% lead.
emission from appliances and equipment used in water
supply installations This product contains substances listed in the candidate list
(date: 17.12.2021) exceeding 0.1 percentage by mass: Lead
2.2 Application
(CAS number 7439-92-1) as a component of the brass alloy
Hand showers are small showers with a handle and not fixed to has been on the candidate list of the Reach Regulation
a wall or (Regulation (EC) No. 1907/2006) since 27.06.2018.
other objects. They can be held in the hand or loosely inserted
into holders. This product/article/at least one partial article contains other
Some hand showers have two or three spray types to choose CMR substances in categories 1A or 1B which are not on the
between, some only candidate list, exceeding 0.1 percentage by mass: no.
have one. They are used for showering or washing off in the
bath tub. Biocide products were added to this construction product or it
has been treated with biocide products (this then concerns a
2.3 Technical Data
treated product as defined by the (EU) Ordinance on Biocide
The technical specifications of the products within the scope of
Products No. 528/2012): no.
the EPD shall be listed, including the reference to the test
methods/test standards for each specification. 2.6 Manufacture
For products with CE marking, the technical specifications must
be specified in accordance with information in the declaration of
performance. The properties relevant to the product should be
specified in the table below. If no information is given for
properties, an explanation must be given in the background
report to the EPD as to why the property is not relevant to the
product.
Constructional data
Name Value Unit
Maximum load temperature
42 °C
permanent operation
Maximum load temperature
70 °C
temporary operation
Flow rate (indications for Depending on flow rate
m3/h
pressure range of 1-3 bar) class 0,54 to 2,28
Sound emissions <30 dB
Performance data of the product with respect to its
characteristics in accordance with the relevant technical
provision (no CE-marking).
2.4 Delivery status
2 Environmental Product Declaration - Hansgrohe Group - Hand Showers
No. 1: The plastic handle of the hand showers is injected.
In addition, all production sites are certified according to the
No. 2: The handle is galvanized with chrome. DIN EN
ISO standards 14001 (environment), 50001 (energy), 45001 (occupational
health and safety) and 9001 (quality). Continuous improvement
of environmental and occupational safety performance is thus
No. 3: The plastic inlet housing is injected. guaranteed.
2.8 Product processing/Installation
The hand showers
No. 4: The plastic pipe bow is injected. are screwed onto the hose by hand with a union nut and a seal
(tools: none).
2.9 Packaging
No. 5: The plastic distributor is injected. For product
protection the hand showers are individually packed in a
cardboard box, which
consists of approximately 80% recycled material. The
No. 6: Meanwhile, the plastic jet body is cardboard is always
injected. printed with lead-free ink and in some cases additionally coated
with clear topcoat.
The inlay of the packaging consists of folded cardboard, fiber
form or plastic
No. 7: The distributor and the jet body are bags, depending on the product.
preassembled. The
packaging can be fully recycled.
No. 8: All the parts are assembled and packed.
All
packaged products fit on a reusable euro pallet.
2.10 Condition of use
Any production waste generated is disposed accordingly. In
To protect
individual cases, the production may differ slightly from the
the hand showers and make them durable, the product is
procedure (for
usually chrome-plated.
example, if the handle is not chrome-plated).
Nevertheless, there are no unhealthy contaminants in the
2.7 Environment and health during manufacturing water. To ensure the
Hansgrohe SE tries to keep the longevity of the product, it should be used and cleaned
impact on people and the environment as low as possible when regularly.
manufacturing its
2.11 Environment and health during use
products.
Our products
Hazards at workplaces are regularly
do not emission any contaminants or substances that are
assessed and reduced to a minimum.
harmful to the
environment or health during the use phase.
2.12 Reference service life
For example, in basic production,
The quality
sawing or grinding work is mainly carried out by robots, and in
and durability of our hand showers is designed for a product life
electroplating,
of about 15
chemicals are dosed automatically via appropriate pump
years. Which on average is approximately the duration of use
stations.
by the consumers. With few
exceptions, all products have a five-year warranty. Furthermore,
an after-sale
service warranty of 15 years is provided.
Emissions that are hazardous to
health are extracted directly at the source and cleaned by filter 2.13 Extraordinary effects
systems. Fire
The products are not classified as
building materials (building products) and are not subject to DIN
4102 and EN
Workplace and emission limits are 13501-1.
regularly monitored and are far below the prescribed limits.
Fire protection
To reduce environmental impact,
water and production waste are recycled wherever possible.
3 Environmental Product Declaration - Hansgrohe Group - Hand Showers
Name Value and reuse it elsewhere.
Building material class
2.15 Disposal
Burning droplets
The waste code of the product is AVV 20 03 01. Disassembly
Smoke gas development of the products consists of the same steps as assembly, in
reverse order.
Water All metal
If a room in which the products offered components can be recycled (as scrap).
by Hansgrohe are installed is flooded with water, the products
are not affected
in their function.
There will be no environmental All plastic
impact. components have a high calorific value and can be sent for
thermal recycling.
Mechanical destruction
If the surface of the coating is
destroyed by a mechanical stress, there is a possibility of
corrosion. In
In the event of mechanical damage, countries where no thermal recycling or substance recycling is
the products may need to be replaced due to possible sharp cut established,
edges. disposal takes place via the waste incineration plant.
2.14 Re-use phase 2.16 Further information
The hand showers are not taken back by the manufacturer for Additional
the purpose of reuse. Users information about our products can be found at
can disassemble the products repeatedly within the reference https://www.hansgrohe.com.
utilization period
3. LCA: Calculation rules
corresponding upstream chains and the actual procurement
3.1 Declared Unit transports. Furthermore, the entire manufacturing phase was
The results of this EPD are valid for the following functional mapped, including the treatment of production waste until the
unit: end-of-waste status (EoW) was reached. Green electricity from
Provide sanitary function for one (1) average hand shower unit hydropower is used for the manufacturing processes in
used in accordance with the manufacturer's recommendations Germany. Green electricity from hydropower and wind power
for a 15-year life, following the manufacturer's operating (50% each) is used for the French production site. US electricity
instructions. An average conditioned hand shower is mix is used for the US production site.
considered the baseline flow. Module A4:
All distribution transports to the customers were considered.
Weighted averaging based on production tonnages in 2020 is Module A5:
chosen as basis for creating the environmental profile. 102 This module covers the installation process with the
different hand showers were considered. corresponding packaging waste generated that needs to be
Functional unit disposed.
Modules B1 & B3-B5:
Name Value Unit
These modules were considered, but evaluated as not relevant
Declared unit 1 pce.
for the products and considered as zero.
Functional unit 1 pce.
Functional unit with packaging 0.34 kg Module B2:
Packaging 0.09 kg
Weight range of the products examined 0.13 - 0.62 kg
Maintenance
Other declared units are allowed if the conversion is shown expenses are declared in this module and consist of weekly
transparently. cleaning expenses
for this product.
For IBU core EPDs (where clause 3.6 is part of the EPD): for
average EPDs, an estimate of the robustness of the LCA Module
values must be made, e.g. concerning the variability of the B6:
production process, geographical representativeness and the
influence of background data and preliminary products This
compared to the environmental impacts caused by the actual module considers the energy input required to bring water to a
production. certain
temperature for the use of a gas low temperature boiler
(scenario B6/1) and for the use of an electric instantaneous
3.2 System boundary
water heater (scenario B6/2).
This representative EPD follows the EPD type "cradle to gate -
with options". The following life cycle modules are declared:
Modules A1-A3:
Module
The product stage begins with considering the production of the
B7:
necessary raw materials and energies, including all
4 Environmental Product Declaration - Hansgrohe Group - Hand Showers
The background datasets used for accounting purposes mainly
This originate from the respective updated GaBi databases at the
module considers the water consumption that can be expected time of calculation. The data for the examined products was
depending on the captured on
function of the product family. the basis of evaluations of internal production and
environmental data, the collection of LCA relevant data within
Modules C1-C4: the supply chain, as well as the evaluation of relevant data for
The modules include the environmental impacts for dismantling the energy supply. The collected
of the products and the treatment of the waste fractions until data were checked for plausibility and consistency. Good
the end-of-waste status (EoW) is reached, including the representativity can be assumed.
associated transports at the end of the product life cycle.
Module D: For the assessment of the variability of the results, all products
were balanced in addition to the average product. See at
chapter 6 for explanation of the variability.
Identification 3.7 Period under review
of the benefits and costs of the product outside the system Life
boundary. For waste, cycle assessment data were collected in 2020.
paper and plastics, these consist of energy credits from thermal
utilization (A3, 3.8 Geographic Representativeness
A5 and C3) in the form of the average European electricity mix Land or region, in which the declared product system is
or thermal energy manufactured, used or handled at the end of the product´s
from natural gas. Recycling of paper, plastic and metal scrap lifespan: Global
results in
credits of the respective raw materials for the primary material
3.9 Allocation
portion of the input. The loads of the waste incineration and
For the production process nearly all raw materials, precursors
recycling processes are assigned to the respective modules
and supplies could be assigned to the declared product.
(A3, A5 and C3) and
Energy, water, galvanization process and production waste
not to module D.
were assigned to the highest value of either the heaviest,
3.3 Estimates and assumptions lightest or most sold product of the product group. No
Energy and water consumption, material amount for coating as byproducts are produced and no allocation is required.
well as waste during production could only be determined on Some of the brass losses from brass processing in module A3
concrete, existing products and not on the average product. are directly reused by Hansgrohe and are modelled as a closed
The highest value of all inputs and outputs for energy, waste loop. Another part of the brass losses (brass particles and
and coating of the top seller, the lightest and the heaviest dusts) is disposed of as waste (without debits and credits).
product was used for the calculation of energy, water, waste Credits for plastics, paper and cardboard recycled in A5 and
and coating. For the incineration with energy recovery (thermal metallurgical waste in C3 are credited in module D.
and electric) of waste, an r1 value of > 0.6 is assumed. The net Credits for the energy recovery of incinerated production waste
efficiency for the average waste incinerated is between 38 % in A1-3, paper, cardboard and plastics in A5 and plastics and
and 44 %, depending on the type of waste respectively the other materials in C3 are credited in module D.
disposal data set. The loads for waste water treatment and waste disposal of core
sand, waste oil and hazardous waste from the manufacturing
3.4 Cut-off criteria phase are allocated to module A3.
The Packaging:
effect associated with the neglected mass shares is less than For paper and cardboard, recycling (91 %) and energy recovery
5% of the (9 %) are considered on a pro rata basis. For plastic, a
effect categories per module. The minimum limit of 1% total proportionate recycling (52 %), energy recovery (48 %)
mass and the use considered, based on Eurostat.
of renewable and nonrenewable primary energy is not Deconstructed product at the end of life:
exceeded. Since the product has a high plastic content, it is assumed that
95% of the plastic and metal components are incinerated (C3)
3.5 Background data and 5% are disposed in landfill (C4). The metal components are
The LCA software GaBi 10.6 was used to model the life cycle. incinerated without energy recovery and the plastic
The entire manufacturing process, as well as energy components are incinerated with energy recovery.
consumption, were modelled on the basis of manufacturer
specific data. 3.10 Comparability
However, generic background datasets were used for the Basically, a comparison or an evaluation of EPD data is only
upstream and downstream processes. The majority of the possible if all the data sets to be compared were created
background datasets used were taken from the current version according to EN 15804 and the building context, respectively
(2021.2) of the GaBi database. Ecoinvent Version 3.6 (2019) the product-specific characteristics of performance, are taken
datasets were only used when suitable GaBi datasets were not into account.
available. The used background database has to be mentioned.
3.6 Data quality
4. LCA: Scenarios and additional technical information
The biogenic carbon content quantifies the amount of biogenic
Characteristic product properties of biogenic carbon carbon in a construction product leaving the factory gate, and it
5 Environmental Product Declaration - Hansgrohe Group - Hand Showers
shall be separately declared for the product and for any
accompanying packaging. In case a reference service life according to applicable ISO
If the total mass of biogenic carbon containing materials is less standards is declared then the assumptions and in-use
than 5 % of the total mass of the product and accompanying conditions underlying the determined RSL shall be declared. In
packaging, the declaration of biogenic carbon content may be addition, it shall be stated that the RSL applies to the reference
omitted. The mass of packaging containing biogenic carbon conditions only.
shall always be declared.
The same holds for a service life declared by the manufacturer.
Corresponding information related to in-use conditions needs
Information on describing the biogenic Carbon Content at
not be provided if a service life taken from the list of service life
factory gate
by BNB is declared.
The biogenic carbon content was calculated based on the
factors from the
Thünen Intitute. Service life
Hansgrohe
Name ValueUnit
SE declares a Service Life of 15 years as an empirical value for
Biogenic carbon content in accompanying kg
0.038 the hand showers when used in accordance with the care
packaging C
instructions.
Note: 1 kg of biogenic carbon is equivalent to 44/12 kg of CO . This
2
value is
The following technical information is a basis for the declared based on their technical service centre's statistics on service
modules. life in
the
Transport to the building site (A4)
market and complaints.
Name ValueUnit
Name Value Unit
Transport distance (Truck) 590 km
Life Span according to the manufacturer 15 a
Capacity utilisation (including empty runs) (Truck) 55 %
Transport distance (Container Ship) 2748 km Operational energy use (B6) and Operational water use
Capacity utilisation (Container Ship) 80 % (B7)
Name Value Unit
Installation into the building (A5)
Water consumption 75.9 m3
No
Energy demand 3535 kWh
additional resources or energy are required for the installation.
The packaging is disposed
End of life (C1-C4)
either by recycling or incineration.
Name Value Unit
Name Value Unit
Collected as mixed construction waste 0.241 kg
Packaging (Paper, cardboard and plastic) 0.095 kg
Energy recovery 0.228 kg
Maintenance (B2) Landfilling 0.012 kg
For
module B2, it is assumed that a weekly cleaning of the product Reuse, recovery and/or recycling potentials (D), relevant
takes place, scenario information
with 0.5 liter of water containing 1.5% soap. The
Name Value Unit energy generated from energy recovery as well as recycled
Maintenance cycle (cleaning) 780 Number/RSL materials are
assigned to module D as possible potentials or avoided loads in
Water consumption/Cycle weekly
0.5 Liter/cycle subsequent systems. Credits are only given for the primary
(cleaning)
portion of
Soap concentration (cleaning) 1.5 %
the inputs.
Water consumption (cleaning) 390 m3
Auxiliary Soap/Tensides (cleaning) 5.85 kg
6 Environmental Product Declaration - Hansgrohe Group - Hand Showers
5. LCA: Results
The following table shows the result of the LCA for 1 piece of an average hand shower. The results in the B-module are based on a
lifetime of 15 years. Scenario B6/1 shows the result for the use of a gas low temperature boiler. Scenario B6/2 shows the result for the
use of an electric instantaneous water heater.
DESCRIPTION OF THE SYSTEM BOUNDARY (X = INCLUDED IN LCA; MND = MODULE OR INDICATOR NOT DECLARED; MNR
= MODULE NOT RELEVANT)
Benefits and
Construction loads beyond
Product stage Use stage End of life stage
process stage the system
boundaries
la ire ta m w a Ry lp p u s tro p s n a rT g n iru tc a fu n a M e h t m o rf tro p s n a rTe tis e h t o t e ta g y lb m e s s A e s U e c n a n e tn ia M ria p e R tn e m e c a lp e R tn e m h s ib ru fe R y g re n e la n o ita re p Oe s u re ta w la n o ita re p Oe s u n o itc u rts n o c -e Dn o itilo m e d tro p s n a rT g n is s e c o rp e ts a W la s o p s iD -e s u e R-y re v o c e R-g n ilc y c e Rla itn e to p
A1 A2 A3 A4 A5 B1 B2 B3 B4 B5 B6 B7 C1 C2 C3 C4 D
X X X X X X X X X X X X X X X X X
RESULTS OF THE LCA - ENVIRONMENTAL IMPACT according to EN 15804+A2: 1 piece average hand shower incl. packaging
Parameter Unit A1-A3 A4 A5 B1 B2 B3 B4 B5 B6/1 B6/2 B7 C1 C2 C3 C4 D
GWP-total kg CO 2 1.08E 2.47E- 1.46E- 0 1.92E 0 0 0 9.44E 1.41E 4.5E+01 0 4.11E-03 4.72E- 7.97E-04 -4.62E-
eq +00 02 01 +01 +02 +03 01 01
GWP-fossil kg CO 2 1.22E 2.46E- 5.89E- 0 1.47E 0 0 0 9.44E 1.41E 4.5E+01 0 4.08E- 4.72E- 7.96E-04 -3.23E-
eq +00 02 03 +01 +02 +03 03 01 01
GWP- kg CO 2 -1.4E-01 0 1.4E-01 0 0 0 0 0 0 0 0 0 0 0 0 -1.38E-
biogenic eq 01
GWP-luluc kg CO 2 2.09E- 1.38E- 1.75E- 0 4.52E 0 0 0 4.78E- 1.99E 3.64E- 0 3.34E- 2.54E- 6.96E-07 -4.47E-
eq 03 04 05 +00 02 +00 02 05 05 04
kg CFC11 2.79E- 4.13E- 5.87E- 8.15E- 4.25E- 8.08E-
ODP 0 0 0 0 3.4E-13 3.36E-11 0 1.3E-10 1.92E-18 -3.1E-10
eq 10 18 17 07 13 19
8.43E- 3.13E- 8.83E- 4.98E- 5.79E- 2.92E 6.83E- 1.89E- -3.65E-
AP mol H+ eq 0 0 0 0 1.11E-01 0 2.44E-06
03 04 06 02 01 +00 06 04 04
EP- 7.36E- 5.18E- 1.44E- 4.36E- 8.61E- 3.77E- 4.79E- 1.22E- 3.76E- -1.42E-
kg P eq 0 0 0 0 0 1.38E-07
freshwater 06 08 08 04 05 03 02 08 08 06
7.48E- 8.64E- 3.13E- 1.14E- 2.46E- 6.95E- 2.69E- 7.97E- -1.28E-
EP-marine kg N eq 0 0 0 0 2.1E-01 0 5.88E-07
04 05 06 02 01 01 06 05 04
7.82E- 9.52E- 3.67E- 1.36E- 2.69E 7.29E 3.31E- 3.08E- 9.56E- -1.36E-
EP-terrestrial mol N eq 0 0 0 0 0 6.2E-06
03 04 05 01 +00 +00 01 05 04 03
kg
2.62E- 2.36E- 7.78E- 4.53E- 7.18E- 1.88E 8.48E- 2.09E- -3.36E-
POCP NMVOC 0 0 0 0 0 6.1E-06 1.85E-06
03 04 06 02 01 +00 02 04 04
eq
4.27E- 1.73E- 8.56E- 1.58E- 5.07E- 4.13E- 5.87E- 3.63E- 3.56E- -1.87E-
ADPE kg Sb eq 0 0 0 0 0 5.44E-11
05 09 10 05 05 04 06 10 09 07
2.62E 3.18E- 3.39E 1.62E 4.63E 5.45E- 2.66E- -4.86E
ADPF MJ 4.9E-02 0 0 0 0 2.5E+04 0 1.14E-02
+01 01 +02 +04 +02 02 01 +00
m3 world
3.19E- 1.68E- 1.76E- 2.47E 2.25E 1.39E -7.14E- -1.33E-
WDP eq 0 5.2E+00 0 0 0 0 3.8E-05 5.4E-02
02 04 03 +00 +02 +01 06 02
deprived
GWP = Global warming potential; ODP = Depletion potential of the stratospheric ozone layer; AP = Acidification potential of land and water; EP =
Eutrophication potential; POCP = Formation potential of tropospheric ozone photochemical oxidants; ADPE = Abiotic depletion potential for non-fossil
resources; ADPF = Abiotic depletion potential for fossil resources; WDP = Water (user) deprivation potential)
RESULTS OF THE LCA - INDICATORS TO DESCRIBE RESOURCE USE according to EN 15804+A2: 1 piece average hand
shower incl. packaging
Parameter Unit A1-A3 A4 A5 B1 B2 B3 B4 B5 B6/1 B6/2 B7 C1 C2 C3 C4 D
4.18E 7.02E 1.42E 1.15E 1.36E -1.61E
PERE MJ 1.32E-021.57E+00 0 0 0 0 0 3.14E-036.95E-02 8.43E-04
+00 +01 +02 +04 +02 +00
1.55E -1.55E
PERM MJ 0 0 0 0 0 0 -1E+00 0 0 0 0 0 0 0
+00 +00
5.73E 7.02E 1.41E 1.15E 1.36E -1.61E
PERT MJ 1.32E-02 1.59E-02 0 0 0 0 0 3.14E-036.95E-02 8.43E-04
+00 +01 +02 +04 +02 +00
2.01E 3.39E 1.62E 4.63E 5.99E -4.86E
PENRE MJ 3.19E-01 1.11E-01 0 0 0 0 2.5E+04 0 5.47E-02 3.13E-01
+01 +02 +04 +02 +00 +00
6.09E -6.21E- -5.72E -3.01E-
PENRM MJ 0 0 0 0 0 0 -1E+00 0 0 0 0 0
+00 02 +00 01
2.62E 3.39E 1.62E 4.63E -4.86E
PENRT MJ 3.19E-01 4.9E-02 0 0 0 0 2.5E+04 0 5.47E-022.66E-01 1.14E-02
+01 +02 +04 +02 +00
SM kg 8.45E-02 0 0 0 0 0 0 0 0 0 0 0 0 0 0 1.28E-02
RSF MJ 7.24E-24 0 0 0 0 0 0 0 0 0 0 0 0 0 0 0
NRSF MJ 0 0 0 0 0 0 0 0 0 0 0 0 0 0 0 0
7 Environmental Product Declaration - Hansgrohe Group - Hand Showers
1.12E -9.12E-
FW m3 6.35E-031.53E-05 4.82E-05 0 1.21E-01 0 0 0 1.58E-01 3.95E-01 0 3.59E-061.29E-03 1.7E-07
+01 04
PERE = Use of renewable primary energy excluding renewable primary energy resources used as raw materials; PERM = Use of renewable primary
energy resources used as raw materials; PERT = Total use of renewable primary energy resources; PENRE = Use of non-renewable primary energy
excluding non-renewable primary energy resources used as raw materials; PENRM = Use of non-renewable primary energy resources used as raw
materials; PENRT = Total use of non-renewable primary energy resources; SM = Use of secondary material; RSF = Use of renewable secondary fuels;
NRSF = Use of non-renewable secondary fuels; FW = Use of net fresh water
RESULTS OF THE LCA – WASTE CATEGORIES AND OUTPUT FLOWS according to EN 15804+A2:
1 piece average hand shower incl. packaging
Parameter Unit A1-A3 A4 A5 B1 B2 B3 B4 B5 B6/1 B6/2 B7 C1 C2 C3 C4 D
-1.51E-
HWD kg 1.78E-061.26E-119.88E-12 0 6.38E-03 0 0 0 3.03E-066.61E-069.53E-08 0 2.88E-125.36E-112.04E-12
09
2.13E 1.77E -2.53E-
NHWD kg 8.86E-024.48E-054.81E-04 0 4.93E-01 0 0 0 7.4E+01 0 8.58E-063.01E-02 1.2E-02
+00 +01 03
3.72E -1.89E-
RWD kg 3.81E-045.13E-072.21E-06 0 3.1E-03 0 0 0 3.58E-02 3.8E-02 0 9.92E-081.29E-051.32E-07
+00 04
CRU kg 0 0 0 0 0 0 0 0 0 0 0 0 0 0 0 0
MFR kg 0 0 8.58E-02 0 0 0 0 0 0 0 0 0 0 0 0 0
MER kg 0 0 0 0 0 0 0 0 0 0 0 0 0 0 0 0
1.11E
EEE MJ 5.05E-02 0 2.27E-02 0 0 0 0 0 0 0 0 0 0 5.07E-05 0
+00
2.01E
EET MJ 1.09E-01 0 4.1E-02 0 0 0 0 0 0 0 0 0 0 0 0
+00
HWD = Hazardous waste disposed; NHWD = Non-hazardous waste disposed; RWD = Radioactive waste disposed; CRU = Components for re-use;
MFR = Materials for recycling; MER = Materials for energy recovery; EEE = Exported electrical energy; EET = Exported thermal energy
RESULTS OF THE LCA – additional impact categories according to EN 15804+A2-optional:
1 piece average hand shower incl. packaging
Parameter Unit A1-A3 A4 A5 B1 B2 B3 B4 B5 B6/1 B6/2 B7 C1 C2 C3 C4 D
Disease 6.26E- 5.05E- 2.48E- 4.02E- 2.47E- 1.24E- 1.22E- -3.17E-
PM 5.74E-11 0 0 0 0 0 4.27E-11 2.44E-11
incidence 08 09 06 06 05 06 09 09
kBq U235 5.14E- 7.47E- 2.49E- 5.69E 6.11E 5.99E 1.45E- 1.32E- 1.89E- -1.91E-
IR 0 1.6E+00 0 0 0 0
eq 02 05 04 +00 +02 +00 05 03 05 02
1.91E 2.35E- 2.67E- 2.22E 1.05E 6.54E 4.04E- 2.99E- 1.05E- -9.78E-
ETP-fw CTUe 0 1.5E+02 0 0 0 0
+02 01 02 +02 +04 +03 02 01 02 01
2.58E- 4.64E- 7.76E- 1.66E- 4.74E- 2.98E- 2.22E- 8.18E- 7.07E- 4.93E- -5.86E-
HTP-c CTUh 0 0 0 0 0
09 12 13 08 08 07 07 13 12 13 11
2.38E- 5.61E- 1.12E- 2.28E- 6.89E- -2.74E-
HTP-nc CTUh 7.4E-08 3.61E-11 0 0 0 0 5E-06 0 4.35E-11 4.21E-11
10 07 05 05 10 09
7.76E 7.74E- 1.92E- 2.38E 9.43E 7.89E 2.29E 1.87E- 6.63E- 8.09E- -2.21E
SQP SQP 0 0 0 0 0
+00 02 02 +02 +01 +03 +02 02 02 04 +00
PM = Potential incidence of disease due to PM emissions; IR = Potential Human exposure efficiency relative to U235; ETP-fw = Potential comparative
Toxic Unit for ecosystems; HTP-c = Potential comparative Toxic Unit for humans (cancerogenic); HTP-nc = Potential comparative Toxic Unit for humans
(not cancerogenic); SQP = Potential soil quality index
Disclaimer 1 – for the indicator “Potential Human exposure efficiency relative to U235”. This impact category deals mainly with the
eventual impact of low-dose ionizing radiation on human health of the nuclear fuel cycle. It does not consider effects due to possible
nuclear accidents, occupational exposure or radioactive waste disposal in underground facilities. Potential ionizing radiation from the
soil, radon and from some construction materials is also not measured by this indicator.
Disclaimer 2 – for the indicators “abiotic depletion potential for non-fossil resources”, “abiotic depletion potential for fossil resources”,
“water (user) deprivation potential, deprivation-weighted water consumption”, “potential comparative toxic unit for ecosystems”,
“potential comparative toxic unit for humans – cancerogenic”, “Potential comparative toxic unit for humans - not cancerogenic”,
“potential soil quality index”. The results of this environmental impact indicator shall be used with care as the uncertainties on these
results are high as there is limited experience with the indicator.
6. LCA: Interpretation
8 Environmental Product Declaration - Hansgrohe Group - Hand Showers
The dominance analysis shows that average product
modules B2, B6 and B7 are the dominant life cycle stages in weighted by production volume.
most of the
categories. The contribution of B2 is due to the demand of soap
and water for
cleaning. Module B6 dominates most of the indicators due to The different types of products all
the energy demand have the same function and differ mainly in terms of design,
for water heating and module B7 has a high contribution to which has an
EPfreshwater influence on construction and materials used. The basic
due to the wastewater treatment. The module A1-A3 has a very structure of the
low contribution product types is always similar. Material type and quantity
to all indicators. proportions do not
The end-of-life stage has no differ much, as also shown in the average material composition
significant influence on the environmental indicators. table.
The environmental burdens from the The deviation of the GWP fossil in
transports (modules A4 and C2) account for less than 1% of the modules A1-C4 has a maximum of 32% and a minimum of -
total burdens of 59% with scenario B6/1
the respective indicators in all cases. (gas low temperature boiler). The variation of the GWP fossil in
modules A1-C4
has a maximum of 32% and a minimum of -60% with scenario
B6/2 (electric
The possible potentials of avoided instantaneous water heater).
loads of subsequent systems (module D) lie outside the
considered system
boundaries and relate exclusively to credits from recycling and
thermal For an average scenario, where 50%
recycling by means of incineration with energy recovery of the of water is heated with gas low temperature boiler and 50%
different with electric
materials. instantaneous water heater, 63% of the hand showers
produced are above the
average GWP fossil value. Whereas 37% reflect the average or
are lower than the
1,795,040 hand showers of 102 average. However, 94% of the ones which are above the
different product types were produced. For the assessment of average just deviate
the variability of between +5 and +25 %.
the results, all products were balanced and compared to the
9 Environmental Product Declaration - Hansgrohe Group - Hand Showers
deviation from the average GWP, the higher the flow rate. The
Modules flow rate ranges
B6 and B7 account for more than 90% of the GWP fossil between 5.2 and 19 l/min. Consequently, the production phase
indicator. The deviation has a minor
from the average is mainly caused by the flow rate in module influence on the LCA results.
B7. The higher the
7. Requisite evidence
The drinking water regulation determines the quality of drinking • Thermoplastic elastomers: Recommendation for the
water at the point of withdrawal. This result in requirements for hygienic assessment of products made of thermoplastic
used materials in drinking water installations in general and elastomers in contact with drinking water (TPE transition
therefore in sanitary fittings in particular. recommendation)
All materials used by Hansgrohe SE, which are in contact with • Ceramics: draft assessment basis for enamels and
drinking water, fulfill the drinking water regulation. ceramic materials: assessment basis for enamels and
Regulations for metals (Europe-wide): ceramic materials in contact with drinking water
(enamel/ceramic assessment basis)
• Acceptance of metallic materials used for products in
• Lubricants: Guideline for the hygienic assessment of
contact with drinking water: 4MS Common Approach
lubricants in contact with drinking water (sanitary
- Part A – Procedure for the acceptance
lubricants), (Lubricant Guideline)
- Part B – 4MS Common Composition List
Regulation for other materials (France):
• Metal recommendation of the federal environment
• ACS: Attestation de Conformité Sanitaire (plastics,
agency: metal materials suitable for drinking water
elastomers, metals)
hygiene
Regulation for other materials (UK):
Regulations for other materials (Germany):
• BS 69 20: Suitability of non-metallic products for use in
• KTW: Assessment basis for plastics and other organic
contact with water intended for human consumption with
materials in contact with drinking water
regard to their effect on the quality of water (plastics,
• Elastomer guideline: Guideline for the hygienic
elastomers)
assessment of elastomers in contact with drinking water
Products of the Hansgrohe SE are therefore uncritical to use
with any drinking water.
8. References
Standards DIN EN ISO 14025: Environmental labels and declarations -
Type III environmental declarations - Principles and procedures,
2011-10
EN 1112 EN 15804
EN 1112:2008 Sanitary tapware - Shower outlets for sanitary DIN EN 15804:2012+A2:2019+AC:2021: Sustainability of
tapware for water supply systems of type 1 and type 2 - construction works - Environmental product declarations - Core
General technical specification rules for the product category of construction products
ISO 3822
ISO 3822: Acoustics – Laboratory tests on noise emission from
appliances and equipment used in water supply installations DIN EN ISO 45001
DIN EN ISO 45001:2018: Occupational health and safety
management systems — Requirements with guidance for use.
DIN 4102-1 2018-03
DIN 4102-1: Fire behaviour of building materials and building
components - Part 1: Building materials; concepts,
requirements and tests. 1998-05 DIN EN ISO 50001
DIN EN ISO 50001:2018: Energy management systems —
Requirements with guidance for use. 2018-08
DIN EN ISO 9001
DIN EN ISO 9001:2015: Quality management systems -
Requirements (ISO 9001:2015) Further References
DIN EN 13501-1 AVV
DIN EN 13501-1:2019-05: Fire classification of construction Draft General administrative provision relating to the Order on
products and building elements - Part 1: Classification using the European list of wastes (Waste List Order – German
data from reaction to fire tests; German version EN 13501- designation: AVV) of 10 December 2001.
1:2018
ECHA
DIN EN ISO 14001 European Chemicals Agency (ECHA) Candidate List of
DIN EN ISO 14001:2015, Environmental management systems Substances of Very High Concern (SVHC) for Authorisation
— Requirements with guidance for use, 2015-09 https://echa.europa.eu/de/candidate-listtable
DIN EN ISO 14025 Ecoinvent
10 Environmental Product Declaration - Hansgrohe Group - Hand Showers
ecoinvent 3.6 Database on Life Cycle Inventories (Life Cycle Instructions for the EPD programme of Institut Bauen und
Inventory data), ecoinvent Association, Zürich, 2020 Umwelt e.V.
Version 2.0, Berlin: Institut Bauen und Umwelt e.V., 2021,
www.ibu-epd.com
EU Ordinance on biocide Products No. 528/2012
European Parliament, 2012. Regulation (EU) no 528/2012 of
the European parliament and of the council of 22 May 2012 PCR Part A
concerning the making available on the market and use of Institut
biocidal products Bauen und Umwelt e.V. (IBU), Product Category Rules for
Building-Related Products and Services. Part A: Calculation
rules for
the life cycle assessment and requirements on the project
report.
Version 2.1, Berlin, 11/2021
Eurostat
PCR Part B
Institut Bauen und Umwelt e.V. (IBU), Requirements on the
Eurostat, last update 26/10/2021 on EPD for fittings and showers. Version 1.1, Berlin, 03/2022
https://ec.europa.eu/eurostat/databrowser/view/ten00063/default/table?
ang=en Thünen Institute
Diestel, Sylvia / Weimar, Holger: Der Kohlenstoffgehalt in
Holz- und Papierprodukten - Herleitung und
GaBi Umrechnungsfaktoren. Thünen
GaBi Working Paper 38. Johann Heinrich von Thünen-Institut.
10.6, GaBi Software System and Database for Life Cycle Hamburg, 2014
Engineering version 2021.2, Sphera Solutions GmbH, The literature referred to in the Environmental Product
Leinfelden-Echterdingen, 1992-2021 Declaration must be listed in full.Standards already fully quoted
in the EPD do not need to be listed here again.
The current version of PCR Part A and PCR Part B of the PCR
IBU 2021 document on which they are based must be referenced.
General
11 Environmental Product Declaration - Hansgrohe Group - Hand Showers
Publisher
Institut Bauen und Umwelt e.V. +49 (0)30 3087748- 0
Hegelplatz 1 info@ibu-epd.com
10117 Berlin www.ibu-epd.com
Germany
Programme holder
Institut Bauen und Umwelt e.V. +49 (0)30 3087748- 0
Hegelplatz 1 info@ibu-epd.com
10117 Berlin www.ibu-epd.com
Germany
Author of the Life Cycle Assessment
brands & values GmbH +49 421 70 90 84 33
Altenwall 14 info@brandsandvalues.com
28195 Bremen www.brandsandvalues.com
Germany
Owner of the Declaration
Hansgrohe Group +49 7836 51-0
Auestr. 5-9 info@hansgrohe-group.com
77761 Schiltach www.hansgrohe-group.com
Germany
12 Environmental Product Declaration - Hansgrohe Group - Hand Showers
