ENVIRONMENTAL PRODUCT DECLARATION
as per ISO 14025 and EN 15804+A2
Owner of the Declaration Xella Baustoffe GmbH
Publisher Institut Bauen und Umwelt e.V. (IBU)
Programme holder Institut Bauen und Umwelt e.V. (IBU)
Declaration number EPD-XEL-20230353-IBA1-EN
Issue date 06/09/2023
Valid to 05/09/2028
Hebel autoclaved aerated concrete, reinforced
Xella Baustoffe GmbH
www.ibu-epd.com | https://epd-online.com
1. General Information
Xella Baustoffe GmbH Hebel autoclaved aerated concrete, reinforced
Programme holder Owner of the declaration
IBU – Institut Bauen und Umwelt e.V. Xella Baustoffe GmbH
Hegelplatz 1 Düsseldorfer Landstraße 395
10117 Berlin 47259 Duisburg
Germany Germany
Declaration number Declared product / declared unit
EPD-XEL-20230353-IBA1-EN 1 m³ autoclaved aerated concrete (AAC) with an average gross density of
528 kg/m³ and including 20 kg reinforcement.
This declaration is based on the product category rules: Scope:
Aerated concrete, 01/08/2021 The LCA is based on the consumption data from three manufacturing
(PCR checked and approved by the SVR) plants of Xella Baustoffe GmbH and the database for 2021.
The owner of the declaration shall be liable for the underlying information
and evidence; the IBU shall not be liable with respect to manufacturer
Issue date information, life cycle assessment data and evidences.
06/09/2023
The EPD was created according to the specifications of EN 15804+A2. In
the following, the standard will be simplified as EN 15804.
Valid to
Verification
05/09/2028
The standard EN 15804 serves as the core PCR
Independent verification of the declaration and data according to ISO
14025:2011
internally X externally
Dipl.-Ing. Hans Peters
(Chairman of Institut Bauen und Umwelt e.V.)
Florian Pronold Matthias Klingler,
(Managing Director Institut Bauen und Umwelt e.V.) (Independent verifier)
1 Environmental Product Declaration - Xella Baustoffe GmbH - Hebel autoclaved aerated concrete, reinforced
2. Product
installed per m³.
2.1 Product description/Product definition
The products under review are reinforced elements of various Sand: The sand used is a natural raw material which contains
formats made of autoclaved aerated concrete (AAC). AAC is quartz (SiO ) as a primary mineral as well as natural minor and
2
classified as a porous, steam-cured, lightweight concrete.
trace minerals. It is an essential base material for the
hydrothermal reaction during steam curing.
(EU) Directive No. 305/2011 (CPR) applies for placing the
product on the market in the EU/EFTA (with the exception of
Cement: In accordance with EN 197-1; cement serves as a
Switzerland). The product requires a Declaration of
binding agent and is largely manufactured from lime marl or a
Performance taking consideration of the DIN EN 12602:2016-
mixture of lime and clay. The natural raw materials are burned
12, Prefabricated reinforced components of autoclaved aerated
before being ground.
concrete standard, and CE marking. Use is governed by the
respective national regulations.
Unhydrated lime: In accordance with EN 459-1; unhydrated
lime serves as a binding agent and is manufactured by burning
2.2 Application
natural lime.
Reinforced components for roofs, ceilings and supporting and
non-supporting walls. Direct contact with water is avoided for
Anhydrite / Gypsum: In accordance with EN 13279-1; the
technical structure reasons.
sulphate agent used serves towards influencing the curing time
2.3 Technical Data for the AAC and originates from natural reserves or is produced
technically.
See the Declaration of Performance for the respective product.
The following table includes general data.
Aluminium: Aluminium powder or paste serves as a pore-
Structural data forming agent. Metallic aluminium reacts in the alkaline
Name Value Unit environment, whereby gaseous hydrogen is formed which
Gross density 350 - 600 kg/m3 generates the pores and then vents after the expansion
process.
Compressive strength 2 - 5 N/mm2
Tensile strength 0.24 - 1.2 N/mm2 Steel: Produced in an electric light arc furnace, manufactured
1000 - to wire rod, connected to steel mats by means of spot welding
Modulus of elasticity N/mm2
3250 and assembled as cages.
Moisture content at 23 °C, 80% < 4 M.-%
Anti-corrosive agents: Anti-corrosive agents prevent
Shrinkage nach EN 680 < 0.4 mm/m
reinforcement corrosion in autoclaved aerated concrete
0.08 -
Thermal conductivity nach EN 12664 W/(mK) components.
0.16
Water-soluble varnishes are used.
Water vapour diffusion resistance factor
5/10 -
nach DIN 4108-4 Water: The availability of water is a fundamental basis for the
Sound insulation acc. to DIN 4109-32 für m' hydraulic reaction undergone by the binding agents. Water is
32-48 [dB]
≤ 150 [kg/m²] also required for manufacturing a homogeneous suspension.
Sound insulation acc. to DIN 4109-32 für
m' > 150 [kg/m²] 48-56 [dB] Mould oil: Mould oil is used as a release agent between the
mould and the raw AAC mixture. PAC (polycyclic aromatic
The product's performance values correspond with the
carbons) are used – free mineral oils plus long-chain additives
Declaration of Performance in terms of its essential properties
for increasing viscosity. This prevents it from running down in
in accordance with DIN EN 12602:2016-12, Prefabricated
the mould and permits economical application.
reinforced components of autoclaved aerated concrete.
Waterproofing agents: Waterproofing agents reduce water
absorption by assembly components and are applied if so
2.4 Delivery status
requested by the customer. Water-soluble methyl siliconates
Products in accordance with EN 12602 and DIN 4223.
are used.
L · W · H
L = max. 8300 mm
The product / At least one partial product contains substances
W = max. 750 mm
from the ECHA list of candidates of Substances of Very High
H = max. 500 mm
Concern (SVHC) exceeding 0.1% by mass: no
2.5 Base materials/Ancillary materials The product / At least one partial product contains other CMR
substances in categories 1A or 1B which are not on the
Name Value Unit
candidate list, exceeding 0.1% by mass in at least one partial
Sand 50–70 % by mass
product: no
Cement (CEM I und CEM II) 15–30 % by mass Biocide products were added to this construction product, or it
Unhydrated lime 8–20 % by mass has been treated with biocide products (this then concerns a
Anhydrite/Gypsum 2–5 % by mass treated product as defined by the (EU) Regulation on Biocide
Products No. 528/2012): no
Aluminium 0,05–0,1 % by mass
Mould oil as an ancillary material
2.6 Manufacture
50 - 70% water by mass (with reference to the solid materials)
is also used. An average of 20 kg reinforced steel is also The ground quartz sand is mixed with unhydrated lime, cement,
small quantities of a sulphate agent in the form of gypsum or
2 Environmental Product Declaration - Xella Baustoffe GmbH - Hebel autoclaved aerated concrete, reinforced
anhydrite, and autoclaved aerated concrete powder (crushed or
ground autoclaved aerated concrete) as production residue, 2.11 Environment and health during use
with the addition of water and aluminium powder or paste, in a In accordance with the current state of knowledge, autoclaved
mixer to form an aqueous suspension and poured into casting aerated concrete does not emit any harmful substances such
moulds. The water slakes the lime under heat generation. as VOC, for example.
Steel reinforcement is manufactured in the autoclaved aerated The naturally ionising radiation of autoclaved aerated concrete
concrete plant. Prior to installation in the casting moulds, the products is extremely low permitting unlimited use of this
reinforcing elements are treated by dipping in anti-corrosive material from a radiological perspective (see 7.1 'Radioactivity').
agent. The aluminium reacts in an alkaline environment,
2.12 Reference service life
whereby gaseous hydrogen is formed which generates the
pores in the raw mixture and vents without residue. The pores Autoclaved aerated concrete displays unlimited resistance
usually have a diameter of 0.5 – 1.5 mm and are exclusively properties when used as designated. The average service life
filled with air. The initial binding process results in semi-solid of solid buildings made of autoclaved aerated concrete
ingots from which the autoclaved aerated concrete components corresponds to that of solid buildings in general. According to
are automatically cut at high accuracy. the available data, the reference service life (RSL) is set at 80
years (Xella 2021).
The final characteristics of the autoclaved aerated concrete are
2.13 Extraordinary effects
formed during the subsequent steam curing process over 6 to
Fire
12 hours at approx. 190 °C and pressure of approx. 12 bar in
In the event of a fire, no toxic gases or vapours can arise.
steam pressure chambers, so-called autoclaves, where the
substances used form calcium silicate hydrates which Fire safety acc. to EN 13501-1
correspond to the mineral tobermorite prevailing in nature. The Name Value
material reaction is concluded on removal from the autoclave.
Building material class A1
The steam is used for other autoclave cycles once the curing
Smoke gas development s1
process is finished. The condensate incurred is used as
process water. This saves energy and avoids pollution by hot Burning droplets d0
steam and waste water.
Water
2.7 Environment and health during manufacturing
When exposed to water (e.g. flooding), autoclaved aerated
The applicable regulations of the professional liability
concrete reacts slightly alkaline. No substances are washed out
associations apply; no special measures need to be taken to
which could be hazardous to water.
protect employee health.
Mechanical destruction
2.8 Product processing/Installation
Not of relevance.
The reinforced AAC elements are processed using lifting gear.
The components are not divided as the reinforced elements are 2.14 Re-use phase
already cut to size in the manufacturing plant. High-speed tools,
Autoclaved aerated concrete offcuts from construction sites can
such as angle grinders, must be equipped with a corresponding
be taken back by the AAC plant via a take-back system. Other
extraction unit as they release fine dust. The AAC components
sorted residual autoclaved aerated concrete can also be taken
are usually connected to the supporting construction using
back by the AAC manufacturers and reused or recycled. This
anchors; in special cases, with thin-bed mortar in accordance
practice has been applied with broken products and
with EN 998-2 or with normal or lightweight mortar.
construction site waste for decades. This material is either
processed as granulate products or added to the AAC mixture
The autoclaved aerated concrete components can be
as a substitute for sand.
plastered, coated or painted. Panelling with small-format parts
in a curtain-type facade or fair-face cavity brickwork in
After the elements of Hebel AAC have been crushed, the
accordance with EN 1996-1-1 is also possible. The
reinforcing steel used can be mechanically or magnetically
corresponding IBU Declarations are to be considered for
separated from the mineral fraction and fed into metal recycling.
assessing mortar, coatings and adhesive.
AAC products are fully recyclable. Based on research results,
The professional liability associations' rules apply. No special
processed AAC demolition material can be used for various
environmental protection measures need to be taken while
recycling paths: e.g. for the bioactivation of autoclaved aerated
processing the building product.
concrete and calcium silicate units (CSU) recycling granulates
with methane-oxidising bacteria to reduce methane outgassing
2.9 Packaging
from domestic waste landfills (Fb 118 2015, Hlawatsch et al.,
Hebel elements are stacked on pallets or squared timbers and
2018).
strapped. Packaging and pallets incurred on the building site
must be collected separately. The reusable wooden pallets are 2.15 Disposal
taken back by the building materials trade (remunerated in the
In accordance with the European Landfill Directive of
German deposit system), which returns them to the autoclaved
27.04.2009 (DepV), valid in Germany, autoclaved aerated
aerated concrete plants.
concrete must be disposed of in Class I landfills (see 7.2
'Leaching').
2.10 Condition of use
Waste key as per EAKV: 17 01 01
As outlined under 2.6 'Manufacturing', autoclaved aerated
concrete primarily comprises tobermorite. It also contains non-
Reinforcing steel itself is practically completely recycled and not
reacting starting components, primarily coarse quartz and
landfilled.
possibly carbonates. Autoclaved aerated concrete recarbonates
Waste key as per EAKV: 17 04 05
for decades after leaving the autoclave. This does not
adversely affect the product properties. The pores are full of air. 2.16 Further information
More information is available at www.ytong-silka.de.
3 Environmental Product Declaration - Xella Baustoffe GmbH - Hebel autoclaved aerated concrete, reinforced
3. LCA: Calculation rules
from packaging treatment.
3.1 Declared Unit
The declared unit is 1 m³ reinforced autoclaved aerated
concrete with a gross density of 528 kg/m³ and 20 kg 3.3 Estimates and assumptions
reinforcement. The average gross density was determined by The product system does not contain any important
averaging the data from the factory production control (FPC), assumptions or estimates with regard to interpretation of the
the amount of reinforcement from the material used in the LCA results. Few auxiliary materials with a combined mass
reference year. share of less than one per cent by mass of the total system
were estimated with technologically similar upstream
Declared unit
processes.
Name Value Unit
Declared unit 1 m3 3.4 Cut-off criteria
Gross density 548 kg/m3 All data from the operating data survey was taken into
consideration in the analysis, i.e. all starting materials used
Conversion factor to 1 kg 0.0018 -
according to the recipe, the thermal energy used, as well as
electricity and diesel consumption.
3.2 System boundary
Specific transport distances were considered for all raw
Type of EPD: cradle to factory gate, with options materials.
Accordingly, material and energy flows accounting for a share
Description of the life cycle phases: < 1% were also considered.
The manufacture of machinery, plants and other infrastructure
Product stage (A1-A3) required for production of the items under review was not taken
Raw material supply and truck transport of raw materials to the into consideration in the LCA.
plant Production expenses, in particular the provision and use It can be assumed that the processes ignored would have
of energy sources and auxiliary materials, as well as packaging contributed less than 5% to the impact categories under review.
materials Treatment of production waste and waste water
Allocation of all environmental burdens by mass between 3.5 Background data
associated co-products (e.g. broken material for use and The software system for comprehensive analysis GaBi 10.5
marketing as cat litter or oil binder) and main product. (GaBi ts) developed by Sphera Solutions GmbH was used for
modelling the manufacture of autoclaved aerated concrete. In
Construction process stage (A4-A5) terms of the background system, GaBi data sets with Content
Module A4: transport by truck to the construction site (100 km). Update (CUP) 2021.1 were used.
Transport distance can be adjusted at building level if
necessary (e.g. for 200 km actual transport distance: 3.6 Data quality
multiplication of the LCA values by a factor of 2). All of the background data sets of relevance for manufacturing
Module A5: Thermal packaging treatment and ensuing credits were taken from the GaBi 10.5 CUP 2021.1 (GaBi ts) software
in module D. Offcuts were not taken into account, as they database. The background data used was last revised less than
strongly depend on the building context. Offcuts can be 3 years ago.
estimated approximately via the declared values for the product
3.7 Period under review
stage (e.g. 5% offcuts: multiplication of the LCA values by a
factor of 0.05). The data basis of the present LCA is based on data recordings
for reinforced autoclaved aerated concrete production from the
Installation of the actual products is usually done using lifting year 2021 in the AAC plants Alzenau, Kringelsdorf and
equipment. The energy required for this is not known. As an Rotenburg located in Germany.
alternative, the same amount of energy is used for assembly as
3.8 Geographic Representativeness
for disassembly (C1).
Land or region, in which the declared product system is
Mortar is not considered in this EPD.
manufactured, used or handled at the end of the product´s
lifespan: Germany
Use stage (B1)
Recarbonation of reactive product components (e.g. CaO). A
recarbonation rate of 95% is assumed (Walther, 2022). 3.9 Allocation
In two of the three plants considered, AAC blocks are produced
End-of-life stage (C1-C4)
in addition to reinforced elements. Raw and auxiliary materials
Module C1: Mechanical demolition (excavator).
are allocated by mass, taking the recipe into account (Walther,
Module C2: transport by truck to waste processing (50 km).
2023).
Transport distance can be adjusted at building level if
In addition, the production process produces broken AAC,
necessary (e.g. for 100 km actual transport distance:
which is further refined into AAC granulate (EPD autoclaved
multiplication of the LCA values by a factor of 2).
aerated concrete granulate). The environmental impacts of
Module C3: (material recycling scenario): waste processing and
autoclaved aerated concrete manufacturing and the waste used
material recycling as fill material (incl. credits for substitution of
for manufacturing AAC granulate were allocated by mass.
gravel in Module D).
During the production process, AAC waste and AAC powder
Module C4: (landfilling scenario): average emissions from
are also incurred which are redirected to the production process
landfilling.
(closed-loop recycling). This internal recycling was considered
in the calculation.
Benefits and loads beyond the system boundaries (D)
Credits from saved expenses through substitution of gravel as 3.10 Comparability
fill material (from Module C3) and credits for energy substitution
4 Environmental Product Declaration - Xella Baustoffe GmbH - Hebel autoclaved aerated concrete, reinforced
Basically, a comparison or an evaluation of EPD data is only the product-specific characteristics of performance, are taken
possible if all the data sets to be compared were created into account. In terms of the background system, GaBi data
according to EN 15804 and the building context, respectively sets with Content Update (CUP) 2021.1 were used.
4. LCA: Scenarios and additional technical information
Characteristic product properties of biogenic carbon Construction installation process (A5)
The analysis includes 2.02 kg of returnable wooden pallets and Packaging materials are thermally treated in Module A5. The
0.33 kg of squared timber (packaging material). credits due to saved expenses are allocated to Module D.
Information describing the biogenic carbon content at the
plant gate Use (B1)
Name ValueUnit See 2.10 Condition of use and 2.12 Reference service life.
kg Name Value Unit
Biogenic carbon content in product -
C Recarbonation rate (Walther 2022) 95 %
Biogenic carbon content in accompanying kg
0.96
packaging C Reference Service Life
Name Value Unit
The following technical information forms the basis for the Life Span according to (Xella 2021) 80 a
declared modules or canbe used for developing specific
End of Life (C1–C4)
scenarios in the context of a buildingevaluation if modules are
not declared (MND). Name Value Unit
Transport to construction site (A4) Diesel consumption for demolition 0,06 kg je dekl.
(excavator) Module C1 Einheit
Name Value Unit
Transport distance to disposal / waste
Litres of fuel 0.597 l/100km 50 km
processing (Module C2)
Transport distance 100 km
Recycling (Module C3, net flow quantity) 532 kg
Capacity utilisation (including empty runs) 61 %
Landfilling (Module C4) 548 kg
Gross density of products transported 549 kg/m3
Further details on the scenarios can be found in section 3.2
'System boundary'.
5 Environmental Product Declaration - Xella Baustoffe GmbH - Hebel autoclaved aerated concrete, reinforced
5. LCA: Results
The environmental impacts of 1 m³ reinforced autoclaved aerated concrete with a gross density of 528 kg/m³ and an additional 20
kg/m³ reinforcement are outlined below. The modules marked 'x' in accordance with EN 15804 in the overview are addressed; the
modules marked 'MND' (Module not declared) do not form a component of the analysis.
The following tables depict the results of the indicators concerning impact estimates, use of resources as well as the waste and other
output flows with reference to the declared unit.
DESCRIPTION OF THE SYSTEM BOUNDARY (X = INCLUDED IN LCA; MND = MODULE OR INDICATOR NOT DECLARED; MNR
= MODULE NOT RELEVANT)
Benefits and
Construction loads beyond
Product stage Use stage End of life stage
process stage the system
boundaries
la ire ta m w a Ry lp p u s tro p s n a rT g n iru tc a fu n a M e h t m o rf tro p s n a rTe tis e h t o t e ta g y lb m e s s A e s U e c n a n e tn ia M ria p e R tn e m e c a lp e R tn e m h s ib ru fe R y g re n e la n o ita re p Oe s u re ta w la n o ita re p Oe s u n o itc u rts n o c -e Dn o itilo m e d tro p s n a rT g n is s e c o rp e ts a W la s o p s iD -e s u e R-y re v o c e R-g n ilc y c e Rla itn e to p
A1 A2 A3 A4 A5 B1 B2 B3 B4 B5 B6 B7 C1 C2 C3 C4 D
X X X X X X MND MNR MNR MNR MND MND X X X X X
RESULTS OF THE LCA - ENVIRONMENTAL IMPACT according to EN 15804+A2: 1 m³ AAC with an average gross density of
528 kg/m³ and including 20 kg reinforcement
Parameter Unit A1-A3 A4 A5 B1 C1 C2 C3 C4 D
GWP-total kg CO 2 eq 2.49E+02 3.36E+00 4.62E+00 -9.03E+01 3.58E-01 1.67E+00 1.47E+00 8.32E+00 -2.62E+00
GWP-fossil kg CO 2 eq 2.52E+02 3.3E+00 4.17E-01 -9.03E+01 3.55E-01 1.64E+00 1.46E+00 8.29E+00 -2.63E+00
GWP-biogenic kg CO 2 eq -3.19E+00 3.56E-02 4.2E+00 0 5.29E-04 1.77E-02 3.76E-03 3.29E-04 1.86E-02
GWP-luluc kg CO 2 eq 1.01E-01 2.73E-02 2.83E-03 0 2.79E-03 1.36E-02 8.01E-03 2.44E-02 -4.91E-03
ODP kg CFC11 eq 6.12E-13 6.59E-16 6.23E-16 0 6.73E-17 3.28E-16 6.52E-15 3.22E-14 -1.94E-14
AP mol H+ eq 2.07E-01 3.54E-03 2.31E-03 0 1.71E-03 1.76E-03 1.36E-02 5.91E-02 -9.45E-03
EP-freshwater kg P eq 1.17E-04 9.91E-06 1.09E-06 0 1.01E-06 4.94E-06 3.33E-06 1.39E-05 -5.1E-06
EP-marine kg N eq 7.23E-02 1.13E-03 9.99E-04 0 8.01E-04 5.63E-04 6.75E-03 1.53E-02 -3.63E-03
EP-terrestrial mol N eq 7.93E-01 1.34E-02 1.17E-02 0 8.87E-03 6.68E-03 7.41E-02 1.68E-01 -3.98E-02
kg NMVOC
POCP 2.15E-01 3.08E-03 2.78E-03 0 2.25E-03 1.53E-03 1.96E-02 4.64E-02 -1.04E-02
eq
ADPE kg Sb eq 1.49E-05 2.96E-07 3.87E-08 0 3.02E-08 1.47E-07 1.61E-06 7.82E-07 -3.29E-07
ADPF MJ 1.88E+03 4.44E+01 5.46E+00 0 4.54E+00 2.21E+01 2.76E+01 1.1E+02 -4.51E+01
m3 world eq
WDP 4.75E+00 3.1E-02 4.42E-01 0 3.16E-03 1.54E-02 2.46E-01 8.9E-01 -1.64E-01
deprived
GWP = Global warming potential; ODP = Depletion potential of the stratospheric ozone layer; AP = Acidification potential of land and water; EP =
Eutrophication potential; POCP = Formation potential of tropospheric ozone photochemical oxidants; ADPE = Abiotic depletion potential for non-fossil
resources; ADPF = Abiotic depletion potential for fossil resources; WDP = Water (user) deprivation potential)
RESULTS OF THE LCA - INDICATORS TO DESCRIBE RESOURCE USE according to EN 15804+A2: 1 m³ AAC with an average
gross density of 528 kg/m³ and including 20 kg reinforcement
Parameter Unit A1-A3 A4 A5 B1 C1 C2 C3 C4 D
PERE MJ 1.84E+02 2.56E+00 3.5E+01 0 2.61E-01 1.27E+00 2.44E+00 1.48E+01 -5.99E+00
PERM MJ 3.46E+01 0 -3.46E+01 0 0 0 0 0 0
PERT MJ 2.19E+02 2.56E+00 4.4E-01 0 2.61E-01 1.27E+00 2.44E+00 1.48E+01 -5.99E+00
PENRE MJ 1.88E+03 4.46E+01 5.48E+00 0 4.56E+00 2.22E+01 2.76E+01 1.1E+02 -4.51E+01
PENRM MJ 0 0 0 0 0 0 0 0 0
PENRT MJ 1.88E+03 4.46E+01 5.48E+00 0 4.56E+00 2.22E+01 2.76E+01 1.1E+02 -4.51E+01
SM kg 3.91E+01 0 0 0 0 0 0 0 5.32E+02
RSF MJ 0 0 0 0 0 0 0 0 0
NRSF MJ 0 0 0 0 0 0 0 0 0
FW m3 2.44E-01 2.93E-03 1.06E-02 0 2.99E-04 1.46E-03 7.16E-03 2.71E-02 -8.27E-03
PERE = Use of renewable primary energy excluding renewable primary energy resources used as raw materials; PERM = Use of renewable primary
energy resources used as raw materials; PERT = Total use of renewable primary energy resources; PENRE = Use of non-renewable primary energy
excluding non-renewable primary energy resources used as raw materials; PENRM = Use of non-renewable primary energy resources used as raw
materials; PENRT = Total use of non-renewable primary energy resources; SM = Use of secondary material; RSF = Use of renewable secondary fuels;
NRSF = Use of non-renewable secondary fuels; FW = Use of net fresh water
RESULTS OF THE LCA – WASTE CATEGORIES AND OUTPUT FLOWS according to EN 15804+A2:
1 m³ AAC with an average gross density of 528 kg/m³ and including 20 kg reinforcement
Parameter Unit A1-A3 A4 A5 B1 C1 C2 C3 C4 D
HWD kg 3.69E-07 2.35E-09 4.07E-10 0 2.4E-10 1.17E-09 1.6E-09 1.17E-08 -6.84E-09
NHWD kg 2.35E+00 7E-03 3.12E-02 0 7.15E-04 3.48E-03 7.95E-03 5.49E+02 -2.22E+01
RWD kg 4.97E-02 8.09E-05 5.94E-05 0 8.27E-06 4.03E-05 2.03E-04 1.16E-03 -3.64E-03
6 Environmental Product Declaration - Xella Baustoffe GmbH - Hebel autoclaved aerated concrete, reinforced
CRU kg 0 0 0 0 0 0 0 0 0
MFR kg 0 0 0 0 0 0 5.48E+02 0 0
MER kg 0 0 0 0 0 0 0 0 0
EEE MJ 0 0 6.13E+00 0 0 0 0 0 0
EET MJ 0 0 1.1E+01 0 0 0 0 0 0
HWD = Hazardous waste disposed; NHWD = Non-hazardous waste disposed; RWD = Radioactive waste disposed; CRU = Components for re-use;
MFR = Materials for recycling; MER = Materials for energy recovery; EEE = Exported electrical energy; EET = Exported thermal energy
RESULTS OF THE LCA – additional impact categories according to EN 15804+A2-optional:
1 m³ AAC with an average gross density of 528 kg/m³ and including 20 kg reinforcement
Parameter Unit A1-A3 A4 A5 B1 C1 C2 C3 C4 D
Disease
PM ND ND ND ND ND ND ND ND ND
incidence
IR kBq U235 eq ND ND ND ND ND ND ND ND ND
ETP-fw CTUe ND ND ND ND ND ND ND ND ND
HTP-c CTUh ND ND ND ND ND ND ND ND ND
HTP-nc CTUh ND ND ND ND ND ND ND ND ND
SQP SQP ND ND ND ND ND ND ND ND ND
PM = Potential incidence of disease due to PM emissions; IR = Potential Human exposure efficiency relative to U235; ETP-fw = Potential comparative
Toxic Unit for ecosystems; HTP-c = Potential comparative Toxic Unit for humans (cancerogenic); HTP-nc = Potential comparative Toxic Unit for humans
(not cancerogenic); SQP = Potential soil quality index
Limitation note 1 – applies to the indicator 'Potential impact of exposure to people to U235':
This impact category mainly addresses the potential impact of low-dose ionising radiation on human health in the nuclear fuel cycle.
This does not consider impacts attributable to possible nuclear accidents and occupational exposure, nor to the disposal of radioactive
waste in underground facilities. Potential ionising radiation from soil, radon and some building materials is also not measured by this
indicator.
Limitation note 2 – applies for the indicators: 'Potential for Abiotic Resource Depletion – Non-Fossil Resources', 'Potential for Abiotic
Resource Depletion – Fossil Fuels', 'Water Depletion Potential (User)', 'Potential Ecosystem Toxicity Comparison Unit', 'Potential
Human Toxicity Comparison Unit – Carcinogenic Effect', 'Potential Human Toxicity Comparison Unit – Non-Carcinogenic Effect',
'Potential Soil Quality Index'.
The results of this environmental impact indicator must be used with caution, as the uncertainties in these results are high or there is
only limited experience with the indicator.
This EPD was created using a software tool.
6. LCA: Interpretation
The manufacturing phase (Modules A1-A3) is of highest atmospheric carbon dioxide during plant growth is shown in
importance for the environmental profile of the product. All connection with the packaging (wooden pallet). Packaging
impact categories with the exception of GWP-biog. are makes moderate contributions in all impact categories.
dominated by the binding agents used.
Relevant contributions to the indicators acidification, resource
The energy sources used are also of great importance for the consumption (minerals and metals), and water consumption
environmental profile. Both the use of thermal energy and arise from the use of aluminium powder.
electrical energy make relevant contributions in all impact
categories. The upstream chain processes from the aggregate used (sand)
make low contributions overall in all impact categories, although
In the case of biogenic global warming potential, the uptake of it is the largest fraction by mass.
7. Requisite evidence
Manufacturer's declarations are available according to which dispenses with a requirement for any additional controls. From
the composition of base materials, the manufacturing process a radiological perspective, the natural radioactivity of the
and product features of the autoclaved aerated concrete building material permits unlimited use thereof.
products under review have remained unchanged since the
evidence outlined below was issued. Accordingly, the evidence 7.2 Leaching performance
applies in full. Leaching by landfilled autoclaved aerated concrete is of
significance for assessing its environmental impact after use.
7.1 Radioactivity LGA 2007, LGA 2011
Method: Measurements of the nuclide content in Bq/kg, Measuring agency: LGA Institut für Umweltgeologie und
determining the Activity Index I Altlasten GmbH, Nuremberg
Summarising report: BfS-SW-14/12, Salzgitter, November Result: All criteria for landfilling in class I landfills are complied
2012 with in accordance with the Landfill Directive DepV dated
Result: The samples were evaluated in accordance with the 27.04.2009 applicable in Germany. In accordance with the
European Commission Guideline "Radiation Protection Council Decision (2003/33/EC) dated 19 December 2002,
112" (Radiological Protection Principles concerning the Natural autoclaved aerated concrete is to be allocated to the 'Non-
Radioactivity of Building Materials, 1999). The Index values I hazardous waste' landfill class.
established are in all cases lower than the exclusion level which
7 Environmental Product Declaration - Xella Baustoffe GmbH - Hebel autoclaved aerated concrete, reinforced
8. References
Standards, directives and regulations materials and products – Determination of thermal resistance
by means of guarded hot plate and heat flow meter methods –
Biocidal Products Regulation Dry and moist products with medium and low thermal
Regulation (EU) No. 528/2012 concerning the making available resistance
on the market and use of biocidal products
EN 13279-1
CPR DIN EN 13279-1:2008-11, Gypsum binders and gypsum
Construction Products Regulation (EU) No 305/2011 of the plasters – Part 1: Definitions and requirements
European parliament and of the Council of 9 March 2011 laying
down harmonised conditions for the marketing of construction EN 13501-1
products and repealing Council Directive 89/106/EEC DIN EN 13501-1:2010-01 +A1:2009: Fire classification of
construction products and building elements – Part 1:
DepV Classification using data from reaction to fire tests
Directive 1999/31/EC on the landfill of waste – Landfill Directive
dated 27 April 2009 (BGBI I, p. 900), last amended by Article 7 EN 15804+A2
V dated 26.11.2010 EN 15804:2012+A2:2019, Sustainability of construction works –
Environmental product declarations – Core rules for the product
DIN 4108-4 category of construction products
DIN 4108-4: 2020-11, Thermal insulation and energy economy
in buildings – Part 4: Technical thermal and moisture protection EN 1996-1-1
rated values DIN EN 1996-1-1: 2013-02, Eurocode 6: Design of masonry
structures – Part 1-1: General rules for reinforced and
DIN 4109-32 unreinforced masonry structures
DIN 4109-32:2016-07, Sound insulation in buildings – Part 32:
Input data for verifying sound insulation by calculation (parts EN 1996-1-1/NA
catalogue) – Solid structures DIN EN 1996-1-1/NA: 2019-12, National Annex - Nationally
determined parameters - Eurocode 6: Design of masonry
DIN 4223 structures – Part 1-1: General rules for reinforced and
DIN 4223-100:2014-12, Application of prefabricated reinforced unreinforced masonry structures
components of autoclaved aerated concrete – Part 100:
Properties and requirements of materials and components EN 1996-2
DIN EN 1996-2 2010-12, Eurocode 6: Design of masonry
EAKV structures – Part 2: Design considerations, selection of
European Waste Catalogue (EWC) in the version of the materials and execution of masonry; German version EN 1996-
Commission Decision 2001/118/EC dated 16 January 2001 2:2006 + AC:2009
amending Decision 2000/532/EC on a waste directory
EN 1996-2/NA
ECHA list DIN EN 1996-2/NA: 2012-01, National Annex - Nationally
Candidate list of Substances of Very High Concern (SVHC) for determined parameters - Eurocode 6: Design of masonry
authorisation (published in accordance with Article 59, structures – Part 2: Design considerations, selection of
paragraph 10 of the REACH Directive), materials and execution of masonry
https://echa.europa.eu/de/candidate-list-table; last amended on
13 December 2021 ISO 14025
DIN EN ISO 14025:2011-10, Environmental labels and
EN 197-1 declarations – Type III Environmental Declarations – Principles
DIN EN 197-1: 2011-11; Cement – Part 1: Composition, and processes (ISO 14025:2006).
specifications and conformity criteria for common cements
PCR: Autoclaved aerated concrete
EN 459-1 Product category rules for building-related products and
DIN EN 459-1: 2010-12, Building lime – Part 1: Definitions, services Part B: Requirements on an EPD for autoclaved
specifications and conformity criteria aerated concrete; version 01.08.2021; Berlin; Institut Bauen
und Umwelt e.V. (pub.); www.ibu-epd.com
EN 680
DIN EN 680: 2005-12; Determination of the drying shrinkage of PCR, Part A
autoclaved aerated concrete Product category rules for building-related products and
services Part A: Calculation rules for the Life Cycle Assessment
EN 998-2 and requirements on the project report, in accordance with EN
DIN EN 998-2:2017-02, Specifications for mortar for masonry – 15804+A2:2019 (version 1.3, 2021 Berlin), Institut Bauen und
Part 2: Masonry mortar; German version EN 998-2:2016 Umwelt e.V. (pub.) www.ibu-epd.com
EN 12602 Directive 2008/98/EC
DIN EN 12602:2016-12, prefabricated reinforced components of the European Parliament and Council dated 19 November
of autoclaved aerated concrete; German version EN 2008 on waste; published on 19 November 2008
12602:2016
Radiation Protection 112
EN 12664 European Commission guideline European Commission:
DIN EN 12664:2001-05, Thermal performance of building Radiological Protection Principles concerning the Natural
8 Environmental Product Declaration - Xella Baustoffe GmbH - Hebel autoclaved aerated concrete, reinforced
Radioactivity of Building Materials, 1999 aerated concrete waste in mortars and lightweight masonry
blocks), Bremen 2018
Other literature
LGA 2007
BfS-SW-14/12 Ch. Kluge: Auslaugtests an Porenbeton zur Bewertung von
K. Gehrke, B. Hoffmann, U. Schkade, V. Schmidt, K. Wichterey: Umweltrisiken im Bezug zu den Geringfügigkeitsschwellen
Natürliche Radioaktivität in Baumaterialien und die daraus (GFS) der LAWA (Leaching tests on AAC for evaluating
resultierende Strahlenexposition (Natural radioactivity in environmental risks in relation to the limit thresholds of the
building materials and the ensuing exposure to radiation), LAWA) (IUA 2007249), LGA Institut für Umweltgeologie und
Federal Office for Radiation Protection, SW-14-/12, Altlasten GmbH, Nuremberg 2007, 19 pages
urn:nbn:de:0221-201210099810, Salzgitter, 2012
LGA 2011
EPD autoclaved aerated concrete granulate Ch. Kluge: Untersuchung von Porenbeton hinsichtlich der
Ytong® - Granulate EPD-XEL-20170148-IAD-1-DE Entsorgung (Testing AAC with regard to disposal)
(IUA2011170), LGA Institut für Umweltgeologie und Altlasten
Fb 118 2015 GmbH, Nuremberg 2011, 10 pages
W. Eden, H. Kurkowski, J.J. Lau, B. Middendorf: Bioaktivierung
von Porenbeton- und Kalksandsteingranulaten mit Walther, 2022
methanoxidierenden Bakterien zur Reduktion von H.B. Walther: CO2 absorption during the use phase of
Methanausgasungen aus Hausmülldeponien – ein Beitrag zum autoclaved aerated concrete by recarbonation, AAC worldwide,
Klima- und Ressourcenschutz – Methanox II (Bioactivation of 1/2022, pp. 18-29
autoclaved aerated concrete and calcium-silicate granulates
with methane-oxidising bacteria to reduce methane outgassing Walther, 2023
from domestic waste landfills – A contribution to climate and H.B. Walther: Calculation of EPD for individual AAC product
resource protection – Methanox II). Research report no. 118 of classes, 2023
Forschungsvereinigung Kalk-Sand e.V. on the AiF research
project 16637 N, Hanover 2015 Xella, 2021
H. Walther: Nutzungsdauer von Porenbeton (Service life of
GaBi ts autoclaved aerated concrete), LB-RS-461, Xella Technologie-
GaBi ts dataset documentation for the software system and und Forschungsgesellschaft mbH, 2021
databases, LBP (University of Stuttgart) and thinkstep AG,
Leinfelden-Echterdingen, 2016 (http://www.gabi- Xella LCA Tool
software.com/deutsch/databases/gabi-databases/) This Declaration is based on calculations by Xella Baustoffe
GmbH using a pre-verified LCA tool based on GaBi Envision:
Hlawatsch et al., 2018 Xella LCA Tool, version 1.0, 2021
F. Hlawatsch, H. Aycil, J. Kropp: Hochwertige Verwertungswege
für Porenbetonbruch in Mörteln und Leichtsteinen aus
Mauerwerk (High-quality recycling routes for autoclaved
9 Environmental Product Declaration - Xella Baustoffe GmbH - Hebel autoclaved aerated concrete, reinforced
Publisher
Institut Bauen und Umwelt e.V. +49 (0)30 3087748- 0
Hegelplatz 1 info@ibu-epd.com
10117 Berlin www.ibu-epd.com
Germany
Programme holder
Institut Bauen und Umwelt e.V. +49 (0)30 3087748- 0
Hegelplatz 1 info@ibu-epd.com
10117 Berlin www.ibu-epd.com
Germany
Author of the Life Cycle Assessment
Sphera Solutions GmbH +49 711 341817-0
Hauptstraße 111- 113 info@sphera.com
70771 Leinfelden-Echterdingen www.sphera.com
Germany
Owner of the Declaration
Xella Baustoffe GmbH 0800 - 5 23 56 65
Düsseldorfer Landstraße 395 info@xella.com
47259 Duisburg www.xella.de
Germany
10 Environmental Product Declaration - Xella Baustoffe GmbH - Hebel autoclaved aerated concrete, reinforced
