ENVIRONMENTAL PRODUCT DECLARATION
as per ISO 14025 and EN 15804+A2
Owner of the Declaration Hilti Aktiengesellschaft
Publisher Institut Bauen und Umwelt e.V. (IBU)
Programme holder Institut Bauen und Umwelt e.V. (IBU)
Declaration number EPD-HIL-20230383-IBA6-EN
Issue date 07.12.2023
Valid to 06.12.2028
HIT-CT 100
HILTI AG
www.ibu-epd.com | https://epd-online.com
1. General Information
HILTI AG HIT-CT 100
Programme holder Owner of the declaration
IBU – Institut Bauen und Umwelt e.V. Hilti Aktiengesellschaft
Hegelplatz 1 Feldkircher Strasse 100
10117 Berlin 9494 Schaan
Germany Liechtenstein
Declaration number Declared product / declared unit
EPD-HIL-20230383-IBA6-EN The declared product is 1kg of HILTI injectable mortar HIT-CT 100
including the packaging.
This declaration is based on the product category rules: Scope:
Reaction resin products, 01.08.2021 The declared product is one kilogram of reaction resin product in the
(PCR checked and approved by the SVR) mixing ratio of the two components necessary for processing. The
packaging is also included in the calculation. The declared unit is stated in
[kg].
Issue date This document refers to the injectable mortar HIT-CT 100 with its
packaging. For the compilation of the life cycle assessment, specific data
07.12.2023
were collected from the factory in Kaufering, Germany, of the HILTI AG.
Since the production of this product has only just started in 2023, no
annual average consumption can be used. The input and output flows
Valid to
used in this calculation were therefore measured directly by the
06.12.2028 manufacturer for this production process for a comparable product.
The owner of the declaration shall be liable for the underlying information
and evidence; the IBU shall not be liable with respect to manufacturer
information, life cycle assessment data and evidences.
The EPD was created according to the specifications of EN 15804+A2. In
the following, the standard will be simplified as EN 15804.
Verification
The standard EN 15804 serves as the core PCR
Independent verification of the declaration and data according to ISO
14025:2011
Dipl.-Ing. Hans Peters
(Chairman of Institut Bauen und Umwelt e.V.) internally X externally
Florian Pronold Matthias Klingler,
(Managing Director Institut Bauen und Umwelt e.V.) (Independent verifier)
1 Environmental Product Declaration - HILTI AG - HIT-CT 100
2. Product
Hilti HIT-CT 100 is stable in terms of a variety of chemical
2.1 Product description/Product definition environmental factors (internal method).
The declared product of HIT-CT 100 is a two component
system. The resin component (component A) comprises a resin 2.4 Delivery status
based on methacrylate as well as mineral and cement like The product Hilti HIT-CT 100 is available in foilpackages with a
fillers. The curing agent component (component B) comprises total of 330 ml and 500 ml injectable mortar in the
peroxide hardener, water and mineral fillers. Mixing the two corresponding mixing ratio.
components A and B in the static mixer initiates the curing
(hardening) reaction of both binder systems. During the curing 2.5 Base materials/Ancillary materials
phase, a very strong bond is formed between the organic and Hilti HIT-CT 100 is supplied in the form of a dual-component
inorganic binder matrix. film-wrapped pack comprising a resin component and a curing
The hybrid system formed during cement and resin curing agent component at a volume ratio of 3:1. The mixing ratio of
results in a crosslinked duromer with desired design properties resin and curing agent components is automatically set during
(high bond strengths within a short curing time) and particular the squeezing process. Product curing commences directly
long-term stability. Composite foils are used for the two- after the components are mixed.
component foil pack of HIT-CT 100. This kind of packaging The product reviewed contains the following component
serves the following purposes: waste volume reduction, easy volumes:
storage and transport, and less packaging material.
For the use and application of the product no legal provisions Resin component:
for harmonizations of the EU exist. Vinyl ester resin mixture: 2.5 to 10 % by weight
Mineral fillers: 40 to 60 % by weight
2.2 Application Cement: 10 to 25 % by weight
Hilti HIT-CT 100 serves for safely securing threaded rods and Other: < 10 % by weight
post-installed rebar connections in dry and damp concrete. It is
approved also for anchoring in uncracked and cracked concrate Curing agent component:
situations. Rebar connections of up to 25 mm can be carried Mineral fillers: 50 to 75 % by weight
out. For anchoring sizes up to 24 mm can be used. Hilti HIT-CT Aluminium oxide: 10 to 25 % by weight
100 is a component of the Hilti SAFEset concept. Hilti SAFEset Water: 10 to 25 % by weight
is a combination of wall plug system components which Dibenzoyl peroxide: < 0.7 % by weight
improve the robustness of fastenings and reduce the Other: < 5 % by weight
possibilities of error during installation. HIT-CT100 is an
injectable mortar for rebar applications and anchoring
fastenings in concrete, it is formulated to minimize health This product article contains substances listed in the ECHA
hazards. candidate list (date: 24.05.2023) exceeding 0.1 percentage by
mass: No
2.3 Technical Data
Constructional data This product contains other carcinogenic, mutagenic, reprotoxic
(CMR) substances in categories 1A or 1B which are not on the
Name Value Unit
candidate list, exceeding 0.1 percentage by mass: No
Density 1845 kg/m3 Biocide products were added to this construction product or it
Compressive strength according to ISO 604 64 N/mm² has been treated with biocide products (this then concerns a
Elastic modules (pressure) according to ASTM treated product as defined by the (EU) Ordinance on Biocide
1877 N/mm²
D695 Products No. 528/2012): No
Hilti HIT-CT 100 displays the following characteristics: 2.6 Manufacture
All raw materials are sourced from Europe. The transport is
Shelf life of 9 months: exclusively by truck. Certain materials go through the required
Container temperature during use: +5 to +40 °C production steps at the supplier, before the final production of
Substrate temperature during installation: -5 to +40 °C (internal the injection mortar in Kaufering. Chemical mortars are usually
method) two-component systems consisting of a binder and a hardener.
The production of chemical mortars consists of a mixing
Open time: process and a filling process of the respective single
-5 to 0 °C 30 min components (binder and hardener) and their subsequent union
+1 to +5 °C 20 min to a two-component system (container). During the mixing
+6 to +10 °C 15 min process control technology is used to weigh and mix solid and
+11 to +20 °C 8 min liquid compounds according to specification. In the next step
+21 to +30 °C 4 min both well-mixed components run through an automized filling
+31 to +40 °C 1.5 min line in which each of the processed masses is filled into a
tubular foil bag. Finally, the single components are united in one
Curing time: container. The two-pack foil bags are packed into cardboard
-5 to 0 °C 6 h boxes and then finally shipped. The manufacturing plant of HIT-
+1 to +5 °C 5 h CT 100, Hilti GmbH Industriegesellschaft für
+6 to +10 °C 4 h Befestigungstechnik, Hiltistr. 6, 86916 Kaufering, Germany, is
+11 to +20 °C 4 h certified according to ISO 9001. The guideline defines
+21 to +30 °C 3.5 h international standards for quality and process management.
+31 to +40 °C 3 h The following flowcharts illustrate the underlying information
modules.
2 Environmental Product Declaration - HILTI AG - HIT-CT 100
product permits safe working conditions in most cases.
2.7 Environment and health during manufacturing
The manufacturing plant of HIT-CT 100, Hilti GmbH 2.12 Reference service life
Industriegesellschaft für Befestigungstechnik, Hiltistr. 6, 86916 Hilti HIT-CT 100 is exposed to a wide variety of environmental
Kaufering, Germany, is certified according to ISO 14001. The factors during the use phase. The anticipated Reference
two guidelines define international standards for quality and Service Life depends on the specific installation situation and
process management as well as for sustainable environmental the exposure associated with the product. The main factors
management. The production site is also certified in influencing the period of use involve weathering as well as
accordance with DIN EN ISO 50001 Energy Management mechanical and chemical loads.
Systems. Description of the influences on the ageing of the product when
applied in accordance with the rules of technology.
2.8 Product processing/Installation
The product is delivered with instructions for use explaining the
basic steps for installation: 2.13 Extraordinary effects
Fire
1) For safe handling the precautionary measures described in Even without any special fire safety features the Injection
the safety data sheet (SDS) (e.g. hand and eye protection) Systems comply with at least the requirements of the EN
must be adhered to 13501-1 standard for fire classes E and Efl. As cross-linked
2) Insert the cartridge into the black cassette methacrylate resins do not melt or drip, the resins do not
3) Screw on the mixing nozzle contribute towards spreading fire. Apart from the common
4) Put the cassette into the dispenser system combustion produces carbon monoxide and carbon dioxide, fire
5) Discard the first trigger pulls gases can contain traces of methyl methacrylate, esters,
6) Fill 2/3 of the borehole with mortar alcohol, and hydrocarbons. Due to the quantities used, they
7) Set the fixing element only have a subordinate influence on the fire characteristics of
a building structure in which they have been installed.
After mixing the components and squeezing the mortar into the
Fire protection
borehole the fixing element has to be set within the working
Name Value
time mentioned in the instructions for use. After the curing time,
described as well in the instructions for use, the mortar is ready Building material class E/Efl
to take up loads. Burning droplets No performance assessed
Smoke gas
2.9 Packaging No performance assessed
development
Hilti HIT-CT 100 is supplied in the form of a 2-foil-pack system
Anchorages satisfy requirements for
and thus leads to very little waste remaining after use on the Reaction to fire
class A1
construction site. After curing, the product can be disposed of
Resistance to fire No performance assessed
with household waste. Full or only partially emptied cartridges
must be disposed of as special waste in accordance with official
regulations. The outer packaging consisting of PE foil and Water
cardboard boxes designed according to the product size can be The cured product is chemically inert and insoluble in water.
recycled. Packaging contaminated by the product must be HIT-CT 100 is certified for use as an anchoring adhesive in
disposed in a safe manner in accordance with local/national concrete for water treatment applications according to NSF.
regulations.
Mechanical destruction
2.10 Condition of use
It is recommended to use dust protection during the demolition
During the installation the temperature of the base material of the cured chemical anchor.
must be between -5°C and +40°C. The temperature of the
product should be between 5 - 25 °C during storage and 5 - 40 2.14 Re-use phase
°C during usage. Hilti literature and official approvals must The product cannot be re-used. After usage, the product can be
always be considered. The two components of HIT-CT 100 are removed by demolition.
only for use in combination with the defined volume ratio and
under these conditions mentioned above to build up a cross- 2.15 Disposal
linked filled duromer. Uncured Hilti HIT-CT 100 can be disposed according to the
European waste code 08 04 09* or 20 01 27*. The built-in cured
2.11 Environment and health during use anchor can be disposed as construction waste for which the
Refer to the Safety Data Sheet (SDS) for detailed information European waste code 17 01 01 applies.
on handling, storage as well as first aid, firefighting and
accidental release measures and disposal considerations. 2.16 Further information
Following the given instructions helps to minimize the risk to Further information is available on request under
health and the environment. Due to its special composition, the anchor.hse@hilti.com and on the Hilti website: www.hilti.group
3. LCA: Calculation rules
declared unit.
3.1 Declared Unit
Declared unit and mass reference
The declared product is an injection mortar from HILTI AG with
the designation HIT-CT 100. The declared unit refers to 1 kg of Name Value Unit
reaction resin product in the mixing ratio of the two components Declared unit 1 kg
required for processing. The packaging, related to 1 kg of
reaction resin product, is additionally included in the calculation 3.2 System boundary
with 0.118 kg. The following table shows the data of the
3 Environmental Product Declaration - HILTI AG - HIT-CT 100
Type of EPD: From cradle to gate with modules C1-C4 and D. Illustration 2: Information moduled A1 to A3 of product
The following information modules are defined as system (part 2)
boundaries in this study:
Production stage (A1- A3):
- A1, raw material extraction,
- A2, transport to the manufacturer,
- A3, production.
End of life (C1- C4):
- C1, deconstruction/demolition,
- C2, transport,
- C3, waste treatment ,
- C4, disposal.
Reuse, recovery and recycling potential (D).
In order to accurately capture the indicators and environmental
impacts of the declared unit, a total of 8 information modules
are considered. The information modules A1 to A3 describe the
material provision, the transport to the production site, as well Illustration 3: Information moduled A1 to A3 of packaging
as the production processes of the product itself.
In the information modules C1 to C4, the deconstruction or
The primary products are sourced from the European Union. demolition from the building, the transport to waste disposal,
The transport is carried out by lorry. The following flow charts the waste treatment and disposal of the product are recorded.
illustrate the underlying production process. Furthermore, reuse, recovery and recycling potentials are
reported in information module D.
3.3 Estimates and assumptions
The electricity mixes and other background data are calculated
country-specifically for the production processes.
For Additives, an assumption was made for the calculation of
material supply. This assumption is based on manufacturer
data. No assumptions or restrictions were made for other recipe
contents or processes.
3.4 Cut-off criteria
All energy and mass inputs were taken into
account.The cut-off criterion according to EN15804+A2 is not
applied.
3.5 Background data
The background data base of the LCA for Expert and ecoinvent
3.9.1 databases, to which this study also refers, is documented
under the following link. (Sphera). http://www.gabi-
software.com/deutsch/index/
Illustration 1: Information module A1 to A3 of product (part
1)
3.6 Data quality
Specific data from the Kaufering plant in Germany of HILTI AG
from 2023 was collected for the preparation of the LCA.HILTI
AG's Kaufering plant in Germany from the year 2023.The
background data from the LCA for Experts database is from the
year from the year 2023 and therefore highly relevant.
The data quality is rated as sufficient.
3.7 Period under review
The input and output flows used in this calculation are from the
year 2023. As this is a new product, no annual average values
can be assumed.
3.8 Geographic Representativeness
Land or region, in which the declared product system is
manufactured, used or handled at the end of the product´s
lifespan: Europe
4 Environmental Product Declaration - HILTI AG - HIT-CT 100
3.9 Allocation 3.10 Comparability
Allocation of co-products takes place in the information Basically, a comparison or an evaluation of EPD data is only
modules A1-A3. possible if all the data sets to be compared were created
The production waste of the injection-moulded according to EN 15804 and the building context, respectively
components is thermally recovered. The electrical and the product-specific characteristics of performance, are taken
thermal energy credits resulting therefrom are into account. The used background data base, mentioned in
completely charged in modules A1-A3. this study, are the LCA for Experts and ecoinvent 3.9.1 data
No further bases
allocations are made.
4. LCA: Scenarios and additional technical information
calculated with a European electricity mix. The construction
Characteristic product properties of biogenic carbon waste is transported by truck 50 km to the waste treatment
No renewable raw materials are used in the product. Therefore, plant. The construction waste is shredded in the waste
the biogeniccarbon is shownas zero. The following raw treatment plant and then dumped.
materials contain biogenic carbon inthe packaging.
Name Value Unit
Information on describing the biogenic carbon content at Collected as mixed construction waste 1 kg
factory gate
Crushing in the shredder 1 kg
Name Value Unit
Landfilling 1 kg
Packaging Cardboard 0,011 kg C
Packaging Paper 0,012 kg C Reuse, recovery and/or recycling potentials (D), relevant
scenario information
In this calculation there are no reuse, recovery and
recyclingpotentials.Therefore, the information module D is
End of life (C1-C4) declared and shown aszero.
The product is demolished using an electric chisel. The Name Value Unit
electrical energy consumption for the tool is assumed to be
Reuse, recovery and recycling potentials 0 kg
0.05 MJ for the declared unit. The electricity consumption is
5 Environmental Product Declaration - HILTI AG - HIT-CT 100
5. LCA: Results
DESCRIPTION OF THE SYSTEM BOUNDARY (X = INCLUDED IN LCA; MND = MODULE OR INDICATOR NOT DECLARED; MNR
= MODULE NOT RELEVANT)
Benefits and
Construction loads beyond
Product stage Use stage End of life stage
process stage the system
boundaries
la ire ta m w a Ry lp p u s tro p s n a rT g n iru tc a fu n a M e h t m o rf tro p s n a rTe tis e h t o t e ta g y lb m e s s A e s U e c n a n e tn ia M ria p e R tn e m e c a lp e R tn e m h s ib ru fe R y g re n e la n o ita re p Oe s u re ta w la n o ita re p Oe s u n o itc u rts n o c -e Dn o itilo m e d tro p s n a rT g n is s e c o rp e ts a W la s o p s iD -e s u e R-y re v o c e R-g n ilc y c e Rla itn e to p
A1 A2 A3 A4 A5 B1 B2 B3 B4 B5 B6 B7 C1 C2 C3 C4 D
X X X MND MND MND MND MNR MNR MNR MND MND X X X X X
RESULTS OF THE LCA - ENVIRONMENTAL IMPACT according to EN 15804+A2: 1 kg HIT-CT 100
Parameter Unit A1-A3 C1 C2 C3 C4 D
Global Warming Potential total (GWP-total) kg CO 2 eq 1.79E+00 4.58E-03 4.36E-03 2.58E-03 1.46E-02 0
Global Warming Potential fossil fuels (GWP-fossil) kg CO 2 eq 1.77E+00 4.53E-03 4.32E-03 2.56E-03 1.46E-02 0
Global Warming Potential biogenic (GWP-biogenic) kg CO 2 eq 2.49E-02 4.91E-05 0 0 0 0
Global Warming Potential luluc (GWP-luluc) kg CO 2 eq 1.34E-03 4.87E-07 3.94E-05 1.92E-05 4.53E-05 0
Depletion potential of the stratospheric ozone layer (ODP) kg CFC11 eq 8.87E-08 8.27E-14 3.73E-16 4.28E-15 3.71E-14 0
Acidification potential of land and water (AP) mol H+ eq 5.33E-03 9.57E-06 1.62E-05 1.34E-05 1.03E-04 0
Eutrophication potential aquatic freshwater (EP-freshwater) kg P eq 3.85E-04 1.67E-08 1.55E-08 8.71E-09 2.93E-08 0
Eutrophication potential aquatic marine (EP-marine) kg N eq 1.23E-03 2.29E-06 7.57E-06 6.13E-06 2.67E-05 0
Eutrophication potential terrestrial (EP-terrestrial) mol N eq 1.3E-02 2.39E-05 8.48E-05 6.77E-05 2.94E-04 0
Formation potential of tropospheric ozone photochemical oxidants kg NMVOC
4.26E-03 6.11E-06 1.46E-05 1.66E-05 8.06E-05 0
(POCP) eq
Abiotic depletion potential for non fossil resources (ADPE) kg Sb eq 6.98E-05 6.95E-10 2.75E-10 2.74E-09 6.72E-10 0
Abiotic depletion potential for fossil resources (ADPF) MJ 3.61E+01 9.43E-02 5.79E-02 5.04E-02 1.94E-01 0
m3 world eq
Water use (WDP) 5.28E-01 9.98E-04 4.91E-05 4.98E-04 1.6E-03 0
deprived
RESULTS OF THE LCA - INDICATORS TO DESCRIBE RESOURCE USE according to EN 15804+A2: 1 kg HIT-CT 100
Parameter Unit A1-A3 C1 C2 C3 C4 D
Renewable primary energy as energy carrier (PERE) MJ 4.1E+00 5.64E-02 4.1E-03 4.68E-03 3.16E-02 0
Renewable primary energy resources as material utilization
MJ 8.6E-01 0 0 0 0 0
(PERM)
Total use of renewable primary energy resources (PERT) MJ 4.96E+00 5.64E-02 4.1E-03 4.68E-03 3.16E-02 0
Non renewable primary energy as energy carrier (PENRE) MJ 3.37E+01 9.43E-02 5.8E-02 5.05E-02 1.94E-01 0
Non renewable primary energy as material utilization (PENRM) MJ 2.52E+00 0 0 0 0 0
Total use of non renewable primary energy resources (PENRT) MJ 3.62E+01 9.43E-02 5.8E-02 5.05E-02 1.94E-01 0
Use of secondary material (SM) kg 6.27E-02 0 0 0 0 0
Use of renewable secondary fuels (RSF) MJ 0 0 0 0 0 0
Use of non renewable secondary fuels (NRSF) MJ 0 0 0 0 0 0
Use of net fresh water (FW) m3 1.5E-02 4.55E-05 4.51E-06 1.44E-05 4.9E-05 0
RESULTS OF THE LCA – WASTE CATEGORIES AND OUTPUT FLOWS according to EN 15804+A2:
1 kg HIT-CT 100
Parameter Unit A1-A3 C1 C2 C3 C4 D
Hazardous waste disposed (HWD) kg 1.86E-08 7.38E-12 2.15E-13 1.31E-13 4.23E-12 0
Non hazardous waste disposed (NHWD) kg 3.94E-02 6.91E-05 8.36E-06 1.33E-05 9.71E-01 0
Radioactive waste disposed (RWD) kg 5.18E-04 1.5E-05 7.5E-08 6.77E-07 2.21E-06 0
Components for re-use (CRU) kg 0 0 0 0 0 0
Materials for recycling (MFR) kg 0 0 0 0 0 0
Materials for energy recovery (MER) kg 0 0 0 0 0 0
Exported electrical energy (EEE) MJ 0 0 0 0 0 0
Exported thermal energy (EET) MJ 0 0 0 0 0 0
RESULTS OF THE LCA – additional impact categories according to EN 15804+A2-optional:
1 kg HIT-CT 100
Parameter Unit A1-A3 C1 C2 C3 C4 D
Disease
Incidence of disease due to PM emissions (PM) ND ND ND ND ND ND
incidence
Human exposure efficiency relative to U235 (IR) kBq U235 eq ND ND ND ND ND ND
Comparative toxic unit for ecosystems (ETP-fw) CTUe ND ND ND ND ND ND
Comparative toxic unit for humans (carcinogenic) (HTP-c) CTUh ND ND ND ND ND ND
Comparative toxic unit for humans (noncarcinogenic) (HTP-nc) CTUh ND ND ND ND ND ND
6 Environmental Product Declaration - HILTI AG - HIT-CT 100
Soil quality index (SQP) SQP ND ND ND ND ND ND
Disclaimer 1 – for the indicator “Potential Human exposure efficiency relative to U235”. This impact category deals mainly with the
eventual impact of low-dose ionizing radiation on human health of the nuclear fuel cycle. It does not consider effects due to possible
nuclear accidents, occupational exposure or radioactive waste disposal in underground facilities. Potential ionizing radiation from the
soil, radon and from some construction materials is also not measured by this indicator.
Disclaimer 2 – for the indicators “abiotic depletion potential for non-fossil resources”, “abiotic depletion potential for fossil resources”,
“water (user) deprivation potential, deprivation-weighted water consumption”, “potential comparative toxic unit for ecosystems”,
“potential comparative toxic unit for humans – cancerogenic”, “Potential comparative toxic unit for humans - not cancerogenic”,
“potential soil quality index”. The results of this environmental impact indicator shall be used with care as the uncertainties on these
results are high as there is limited experience with the indicator.
6. LCA: Interpretation
The dominance analysis shows that the main causes of Illustration: Dominance analysis A1
environmental impacts and indicators are to be found in
information module A1. This is shown by the total global
warming potential for material supply with approx. 90 %, related Within the reaction resin mixture itself, the material supply of
to all information modules. For the total non-renewable primary the Methacrylate Diluent generates approx. 38 % of the total
energy it is about 94 %. global warming potential and approx. 47 % of the total non-
renewable primary energy. The Methacrylat Resin has a share
of approx. 27 % of the total greenhouse gas emissions and
approx. 27 % of the total non-renewable primary energy.
Illustration: Dominance analysis A1- A3
Illustration: Dominance analysis A1, injectable
If we look at the material supply of the reaction resin mixture mortar mixture
and the packaging in detail, it becomes clear which raw
materials contribute decisively to the respective environmental
impacts and indicators.The reactive resin mixture itself has a
share of 89 % of the total global warming potential in
information module A1. Approx. 2 % is accounted for by the
Polyethylene High-Density PE-HD and approx. 2 % by the
Polypropylene PP.
7. Requisite evidence
Hilti HIT-CT 100 complies with the requirements of
• emission class A+ outlined in the French VOC Directives
• DIBt (2018) in combination with the NIK values from
in accordance with the Eurofins attestation,
AgBB (2021) for applications in interior areas,
7 Environmental Product Declaration - HILTI AG - HIT-CT 100
Both in accordance with the Eurofins test report, No. 392-2022- DIBt/AgBB overview of results (3 days [μg/m³])
00544102_A_EN. Name Value Unit
AgBB overview of results (28 days [µg/m³]) TVOC (C6 - C16) < 10000 μg/m3
Name Value Unit Carcinogenic Substances < 10 μg/m3
TVOC (C6 - C16) < 1000 μg/m3
Sum SVOC (C16 - C22) < 100 μg/m3
R (dimensionless) < 1 -
VOC without NIK < 100 μg/m3
Carcinogenic Substances < 1 μg/m3
8. References
DIN EN 196-1 Candidate List of substances of very high concern for
DIN EN 196-1: 2016-11, Prüfverfahren für Zement - Teil 1: Authorisation European Cheminals Agency (ECHA), in
Bestimmung der Festigkeit accordance with Article 50(10) of the REACH regulation
DIN EN 14293 DIBt (2010)
DIN EN 14293: 2006-10, Klebstoffe - Klebstoffe für das Kleben Grundsätze zur gesundheitlichen Bewertung von Bauprodukten
von Parkett auf einen Untergrund - Prüfverfahren und in Innenräumen (Oktober 2010)
Mindestanforderungen
Eurofins test report, No. 392-2022-00544102_A_EN
EN 13501-1
EN 13501-1: 2019-05, Eurofins test report, No. 392-2022-00544102_A_EN VOC
Klassifizierung von Bauprodukten und Bauarten zu ihrem test report for verification of compliance with the French
Brandverhalten - Teil 1: Klassifizierung mit den Ergebnissen directive from 2010
aus den Prüfungen zum Brandverhalten von Bauprodukten
Eurofins test report, No. 392-2021-00413601_H_EN VOC
EN 15804 test report for verification of compliance with
EN 15804+A2:2019+AC:2021, Sustainability of construction CDPH/EHLB/Standard Method V1.2 from 2017
works — Environmental Product Declarations — Core rules for
the product category of construction products European Waste code in accordance with the European
Waste Catalogue (EWC) (EWC 2014/955/EU) Commission
ISO 9001 Decision amending Decision 2000/532/EC on the list of waste
ISO 9001: 2015-11, Qualitätsmanagementsysteme - pursuant to Directive 2008/98/EC of the European Parliament
Anforderungen and of the Council
ISO 14001 French VOC Directives Décret no 2011321 du 23 mars 2011
ISO 14001: 2015-09, Umweltmanagementsysteme - relatif à l'étiquetage des produits de construction ou de
Anforderungen mit Anleitung zur Anwendung revêtement de mur ou de sol et des peintures et vernis sur
leurs émissions de polluants volatils Arrêté du 19 avril 2011
ISO 14025 relatif à l'étiquetage des produits de construction ou de
DIN EN /ISO 14025:2011-10/, Environmental labels and revêtement de mur ou de sol et des peintures et vernis sur
declarations — Type III environmental declarations — leurs émissions de polluants volatils
Principles and procedures
NSF
ISO 50001 NSF/ANSI/CAN 61 Drinking Water System Components Health
ISO 50001: 2018-08, Energiemanagementsysteme - Effects
Anforderungen mit Anleitung zur Anwendung
Calculation rules: PCR - Part A
EN ISO 604 Institut Bauen und Umwelt e.V. (IBU), 2022. Product Category
EN ISO 604: 2003-12, Kunststoffe - Bestimmung von Rules for Building-Related Products and Services. Part A:
Druckeigenschaften Calculation rules for the life cycle assessment and
requirements on the project report. Version 1.3 (08.2022)
AgBB (2021)
Vorgehensweise bei der gesundheitlichen Bewertung der ecoinvent 3.9.1
Emissionen von flüchtigen organischen Verbindungen (VVOC, Backgroun data: ecoinvent 3.9.1
VOC und SVOC) aus Bauprodukten (2021) Zürich: ecoinvent
http://www.ecoinvent.org
ASTM D695 (06.06.2023)
ASTM D695: 2015-00: Standard Test Method for Compressive
Properties of Rigid Plastics IBU 2021
General Instructions for the EPD programme of Institut Bauen
CDPH/EHLB/Standard Method V1.2 California CDPH und Umwelt e.V. Version 2.0,
Standard Method is a US standard for evaluating and restricting Berlin: Institut Bauen und Umwelt e.V.,2021
VOC emissions to indoor air. Developed in California as www.ibu-epd.de
"Section 01350" Specification, several systems in the US refer
to CDPH Standard Method Product category rules for construction products – Part B
Reaction resin products, 08.2021
8 Environmental Product Declaration - HILTI AG - HIT-CT 100
(06.06.2023)
The literature referred to in the Environmental Product
Sphera Declaration must be listed in full.Standards already fully quoted
LCA for Experts in the EPD do not need to be listed here again.
Leinfelden-Echterdingen; Sphera Solution GmbH, The current version of PCR Part A and PCR Part B of the PCR
https://gabi.sphera.com/databases/gabi-data-search/ document on which they are based must be referenced.
9 Environmental Product Declaration - HILTI AG - HIT-CT 100
Publisher
Institut Bauen und Umwelt e.V. +49 (0)30 3087748- 0
Hegelplatz 1 info@ibu-epd.com
10117 Berlin www.ibu-epd.com
Germany
Programme holder
Institut Bauen und Umwelt e.V. +49 (0)30 3087748- 0
Hegelplatz 1 info@ibu-epd.com
10117 Berlin www.ibu-epd.com
Germany
Author of the Life Cycle Assessment
FIT-Umwelttechnik GmbH 05362 72 69 474
Westerstr. 13 bertram@fit-umwelttechnik.de
38442 Wolfsburg www.fit-umwelttechnik.com
Germany
Owner of the Declaration
Hilti Aktiengesellschaft +423 234 2111
Feldkircher Strasse 100 HAGHSE@hilti.com
9494 Schaan www.hilti.com
Liechtenstein
10 Environmental Product Declaration - HILTI AG - HIT-CT 100
