Environmental Product Declaration
according to ISO 14025 and EN 15804+A2
Owner oft he declaration: RIVA ACIER S.A.S.
Publisher: Kiwa – Ecobility Experts
Program operator: Kiwa – Ecobility Experts
Declaration number: EPD-RIVA ACIER-175-EN
Issue date: 27.01.2022
Valid to: 27.01.2027
Hot Rolled concrete reinforcing bars
This average EPD is based on the LCA of reinforcing steel bars from RIVA ACIER S.A.S., which is pro-
duced in the steel mills and rolling mills of Iton Seine (Bonniéres) and Alpa (Limay Porcheville).
1. Genereal information
RIVA ACIER S.A.S. Hot Rolled concrete reinforcing
bars
Program operator: Owner of the declaration:
Kiwa – Ecobility Experts RIVA ACIER S.A.S.
Voltastr. 5 Immeuble ALPA
13355 Berlin ZI Limay Porcheville
Deutschland 78440 Gargenville
France
Declaration number: Declared product / declared unit:
EPD-RIVA ACIER-175-EN 1 kg concrete reinforcing steel bars
Issue date: Valid until:
27.01.2022 27.01.2027
Scope: Product category rules:
This average EPD is based on the LCA of the PCR B for construction steel products (con-
hot rolled reinforcing steel bars from RIVA struction steel products; draft; 2020-03-13).
ACIER S.A.S., which is produced in the steel
mills and rolling mills of Iton Seine (Bon- Verification:
niéres) and Alpa (Limay Porcheville). The CEN Norm EN 15804+A2 serves as the
The owner of the declaration shall be liable core PCR.
for the underlying information and evidence. Independent verification of the declaration
Kiwa – Eco-bility Experts shall not be liable and data according to ISO 14025
with respect to manufacturer information, ☐internally ☒externally
life cycle assessment data and evidences.
Frank Huppertz Julian Rickert
(Head of Kiwa – Ecobility Experts) (Extern verfifier of GreenDelta GmbH)
Prof. Dr. Frank Heimbecher
(Chairman of the independent expert committee - Eco-
bility Experts)
RIVA ACIER S.A.S. – EPD Hot Rolled concrete reinforcing bars | Seite 2
2. Product
2.1 Product description
The product to be declared is hot rolled concrete reinforcing bars from RIVA ACIER S.A.S., which is
produced in the steel mills and rolling mills of Iton Seine (Bonniéres) and Alpa (Limay Porcheville).
2.2 Application
The hot rolled concrete reinforcing bars is used for the reinforcement of concrete.
2.3 Technical data
The following technical data was provided by RIVA ACIER S.A.S..
Table 1: Technical data
Parameter Value
Steel Grade B450C, B500B, B500C
Yield strength 450 to 500 MPa
Ratio R /R at least 1.08 (class B) to at least 1.15 (class C)
m e
Way of production EAF
Standard/Norm EN 10080 + all national standards for each European country
Range of diameters 8 to 40 mm
2.4 Manufacturing
Concrete reinforcing bar is hot rolled and heat treated from the rolling heat. The product is supplied
in different lengths as technically straight ribbed bar.
2.5 Raw materials
Table 2 lists the raw materials for the steel billets from which the hot rolled reinforcing steel bars is
made, with the average shares in mass percent. To respect the commercial secrets, the values are
given in intervals that represents the distribution of the shares of the raw materials.
Table 2: Raw materials and shares in mass percent
Material Share in m%
Ferrosilicon 0-2
Limestone 1-3
Manganese for Siliconmanganese 0-2
Petroleum Coke 0-2
Scrap 95-98
Silicon for Silicomanganese 0-2
2.6 Reference service life
Since the service life of reinforcing steel is not considered, there is no need to specify a reference ser-
vice life.
RIVA ACIER S.A.S. – EPD Hot Rolled concrete reinforcing bars | Seite 3
3. LCA: Calculation rules
3.1 Declared unit
According to PCR B for construction steel products (draft; 2020-03-13), the declared unit is 1 kg of
concrete reinforcing steel bars.
Table 3: Declared unit
Parameter Value Unit
Declared unit 1 kg
For the calculation of potential environmental impacts, process-specific data were collected for the
product under consideration. All the energy and materials required for the production process were
determined, as were the data for calculating the auxiliary materials and co-products.
This is an average EPD for hot rolled reinforcing steel bars, which were produced at the plant locations
Iton Seine (Bonniéres) and Alpa (Limay Porcheville). The range of diamters is from 8mm to 40mm. The
average is calculated on the basis of the 2020 production volume and the shares shown in Table 4.
Table 4: Shares of the products in the product group "Hot Rolled reinforcing steel bars" based on production
volume
Plant Location Production volume 2020 in kg Share in %
Iton Seine (Bonniéres) 279 989 000 44.8
Alpa (Limay Porcheville) 344 805 140 55.2
3.2 System boundary
In this life cycle assessment according to EN 15804+A2, the following phases of the product life cycle
are considered:
A1: Extraction and processing of raw materials and processing of secondary materials used as input
(e.g. recycling processes)
A2: Transport to Manufacturing
A3: Manufacturing
C2: Transport to waste treatment
C3: Waste treatment for reuse, recovery and/or recycling
C4: Disposal
D: Reuse-, Recovery-, Recycling- potentials, indicated as net flows and benefits
Therefore, the type of this average EPD is “from cradle to gate with options”.
For the declared life cycle phases, all inputs (raw materials, precursors, energy and auxiliary materials)
as well as the waste generated were considered.
3.3 Estimates and assumptions
The raw materials were assigned the waste scenario for reinforcing steel "Steel, reinforcement" both
for waste during production and at the end of product life. The waste scenario is based on the "Natio-
nale Milieudatabase" (NMD), the national environmental database of the Netherlands. This is due to
the fact that the used online EPD tool "R<THiNK" was developed by Nibe in the Netherlands. The waste
scenario used for reinforcing steel has the NMD ID 72. Further information is listed in chapter 4. A
RIVA ACIER S.A.S. – EPD Hot Rolled concrete reinforcing bars | Seite 4
suitable waste scenario from the NMD database was chosen and assigned for each of the auxiliary
materials and listed in chapter 4.
3.4 Period under review
All product- and process-specific data were collected for the 2020 operating year and are thus up-to-
date.
3.5 Cut-off criteria
For the process modules A1 to A3, all process-specific data were collected. Potential environmental
impacts were assigned to the material flows based on the Ecoinvent database V3.6 of 2019. All flows
contributing to more than 1 percent of the total mass, energy, or environmental impacts of the system
were considered in the LCA. It can be assumed that the neglected processes would have contributed
less than 5 percent to the considered impact categories
3.6 Data quality
To ensure the comparability of the results, only consistent background data from the Ecoinvent data-
base V3.6 of 2019 were used in the LCA (e.g. data sets on energy, transports, auxiliary and operating
materials). The database is regularly checked and thus complies with the requirements of EN 15804
(background data not older than 10 years). Almost all consistent data sets contained in the Ecoinvent
database V3.6 of 2019 are documented and can be viewed in the online documentation.The data refer
to the annual average of inputs (energy, inputs, etc.) consumed during the operating phase 01/2020 -
12/2020 and were converted to reference flows (input / output per declared unit).
The general rule was followed that specific data from specific production processes or average data
derived from specific processes must have priority in the calculation of an LCA. Data for processes over
which the manufacturer has no control were assigned generic data.
The calculation of the LCA was performed using the online EPD tool "R<THiNK" from Nibe.
3.7 Allocation
The allocation regarding production waste is explained in the project report of this average EPD. There
are no multi-functional processes to be considered. Specific information on allocations within the back-
ground data can be found in the Ecoinvent database V3.6 document of 2019.
3.8 Comparability
Basically, a comparison or an evaluation of EPD data is only possible if all the data sets to be compared
were created according to EN 15804 and the building context, respectively the product-specific char-
acteristics of performance, are considered. The results of the LCA must be considered as average val-
ues out of different plant locations. To compare specific data for different plant locations in a direct
way it is necessary to run the calculation for the LCA separately.
3.9 Data collection
For the data collection, ISO 14044 section 4.3.2 was considered.
The objective and the scope of the study were defined in consultation with RIVA ACIER S.A.S.. The data
collection was implemented by using an Excel data collection template provided by Kiwa GmbH. The
data collected was checked by Kiwa GmbH, for example by checking the extent to which the data for
the different production processes matched to each other. In this way, some errors (e.g. unit errors)
could still be corrected in cooperation with RIVA ACIER S.A.S.. The annual values were then related to
the declared unit of one kilogram of steel product with the aid of corresponding calculations.
RIVA ACIER S.A.S. – EPD Hot Rolled concrete reinforcing bars | Seite 5
3.10 Calculation methods
The calculation procedures described in ISO 14044 Section 4.3.3 were used for the life cycle assess-
ment. The evaluation is based on the phases according to the system boundaries and the processes
contained.
RIVA ACIER S.A.S. – EPD Hot Rolled concrete reinforcing bars | Seite 6
4. LCA: Scenarios and additional technical information
As previously explained, the NMD waste scenario "Steel, reinforcement" with ID 72 was used for the
raw material waste streams. For each of the auxiliary materials, a suitable waste scenario from the
NMD database was chosen and assigned.
Table 5: C2 – Transport End of Life
Waste Transport
Waste Scenario Transport Profile
Treatment ditance in km
Landfill Lorry (Truck), unspecified (default) 100
concrete (i.a. elements,
brickwork, reinforced con- Incineration Lorry (Truck), unspecified (default) 150
crete) (NMD ID 7)
Recycling Lorry (Truck), unspecified (default) 50
Landfill Lorry (Truck), unspecified (default) 100
Lubricating oil (landfill)
ID: WDE0003-8432 Incineration Lorry (Truck), unspecified (default) -
Recycling Lorry (Truck), unspecified (default) -
Landfill Lorry (Truck), unspecified (default) 100
finishes (adhered to wood,
Incineration Lorry (Truck), unspecified (default) 150
plastic, metal) (NMD ID 1)
Recycling Lorry (Truck), unspecified (default) 50
Landfill Lorry (Truck), unspecified (default) 100
Steel, reinforcement (NMD
Incineration Lorry (Truck), unspecified (default) 150
ID 72)
Recycling Lorry (Truck), unspecified (default) 50
Landfill Lorry (Truck), unspecified (default) 100
wood 'clean', via residue
Incineration Lorry (Truck), unspecified (default) 150
(NMD ID 35)
Recycling Lorry (Truck), unspecified (default) 50
Table 6: C4 – Shares of waste treatment
Shares of waste treatment [%]
Waste Scenario
Landfill Recycling Incineration
concrete (i.a. elements, brickwork, rein- -
1 99
forced concrete) (NMD ID 7)
Lubricating oil (landfill) -
100 -
ID: WDE0003-8432
finishes (adhered to wood, plastic, metal) 100
- -
(NMD ID 1)
Steel, reinforcement (NMD ID 72) 5 95 -
wood 'clean', via residue (NMD ID 35) 10 5 85
RIVA ACIER S.A.S. – EPD Hot Rolled concrete reinforcing bars | Seite 7
Table 7: D – Used Environmental Profile for loads
Used Environmental Profile for loads
Material Waste Scenario
Landfill Recycling Incineratiom
Ferrosilicon
Covering Powder
Lime
Scrap steel
{Europe without Materials for
Manganese for
Switzerland} | recycling, no
Siliconmangaese Steel, reinforce-
treatment of waste pro- -
ment (NMD ID 72)
scrap steel, inert cessing taken
Petroleum Coke
material landfill | into account
Scrap Cut-off
Silicon for
Silicomanganese
Cast Iron Rolls
Argon
Waste paint {Eu-
rope without
Dolomite
finishes (adhered Switzerland}|
Electrodes to wood, plastic, - - treatment of
metal) (NMD ID 1) waste paint, mu-
Nitrogen
nicipal incinera-
tion | Cut-off
Refractory
Waste concrete
{Europe without
concrete (i.a. ele-
Switzerland}| Crushing, per
ments, brickwork,
Bauxite treatment of kg stoney ma- -
reinforced con-
waste concrete, terial
crete) (NMD ID 7)
inert material
landfill | Cut-off
Sodium Hydroxide
for Water
Treatment
Lubricating oil
(landfill) Lubricating oil |
Light Fuel Oil - -
ID: WDE0003-8432 production (EU)
Lubricating Oil
RIVA ACIER S.A.S. – EPD Hot Rolled concrete reinforcing bars | Seite 8
Waste wood, un-
Wood chip-
treated {Europe
ping, industrial Waste wood, un-
without Switzer-
wood 'clean', via residual wood, treated {CH}|
land}| treatment
Wood Packaging residue (NMD ID stationary elec- treatment of,
of waste wood,
35) tric chipper municipal incin-
untreated, sani-
{GLO}| market eration | Cut-off
tary landfill | Cut-
for | Cut-off
off
Table 8: D – Used Environmental Profile for benefits
Used Environmental Profile for benefits
Waste Scenario
Landfill Recycling Incineration
concrete (i.a. elements, brickwork, Gravel, round
- -
reinforced concrete) (NMD ID 7) (RoW)
Lubricating
Lubricating oil (landfill)
oil | produc- - -
ID: WDE0003-8432
tion (EU)
0267-avD&Verme-
den energieproduc-
tie AVI, o.b.v. FOS-
finishes (adhered to wood, plastic,
- - SIELE grondstoffen,
metal) (NMD ID 1)
18% elektrisch en
31% thermisch (per
MJ LHV)
Benefits module D
| World Steel
method (Steel pro-
Steel, reinforcement (NMD ID 72) – duction, electric, -
low-alloyed - Steel
production, con-
verter, unalloyed)
Avoided energy pro-
duction incinerator,
Wood chips, dry, based on RENEWA-
wood 'clean', via residue (NMD ID 35) - measured as dry BLE raw materials,
mass (EU) 18% electrical and
31% thermal (per MJ
LHV)
RIVA ACIER S.A.S. – EPD Hot Rolled concrete reinforcing bars | Seite 9
5. LCA: Results
The following tables show the results of the life cycle assessment, more precisely for the environmental
impact indicators, resource consumption, output flows and waste categories. The results presented
refer to the declared unit of 1 kg of hot rolled concrete reinforcing bars. Since the installation of the
product A5 is not considered, the demolition C1 is not considered either.
The results of the environmental impact indicators ETP fw, HTP-c, HTP-nc, SQP, ADP-f, ADP-mm and
WDP must be used with caution, as the uncertainties in these results are high or as there is limited
experience with the indicator.
The IRP impact category mainly addresses the potential effect of low-dose ionizing radiation on human
health in the nuclear fuel cycle. It does not consider effects due to possible nuclear accidents and oc-
cupational exposure, nor does it consider radioactive waste disposal in underground facilities. Poten-
tial ionizing radiation from soil, radon, and some building materials is also not measured by this indi-
cator.
Table 9: Overview of the considered information modules showing all phases of the building life cycle according
to DIN EN 15804 (X = module declared)
Description of the system boundary (X = Included in LCA)
Benefits and
Construction loads beyond the
Product stage Use stage End of life stage
process stage system bounda-
ries
y lp p u s la ire ta m w a
R
tro p s n a rT g n iru tc a fu n a M m o rf tro p s n a rTre r uu nt ac o mat -f e s u fo e c a lp n o itc u r- tl sa nts on C-is s e c o rp n o ita l e s U e c n a n e tn ia M ria p e R tn e m e c a lp e R n e m h s ib ru fe R / n o itc u rts n eo Dc -n o itilo m e d tro p s n a rT g n is s e c o rp e ts a W la s o p s iD y re ev o s uc ee RR -- gla ni it ln c ye cto e Rp -
A1 A2 A3 A4 A5 B1 B2 B3 B4 B5 C1 C2 C3 C4 D
X X X - - - - - - - - X X X X
RIVA ACIER S.A.S. – EPD Hot Rolled concrete reinforcing bars | Seite 10
Table 10: Results of the LCA – Environmental impact categories
Results of the LCA – Environmental impact categories
Impact
Unit A1 A2 A3 C2 C3 C4 D
category
AP mol H+ eqv. 1,75E-04 9,15E-05 1,03E-03 4,57E-05 0,00E+00 2,78E-06 4,23E-04
GWP-to-
kg CO2 eqv.
tal 2,09E-02 1,43E-02 2,43E-01 7,89E-03 0,00E+00 2,93E-04 8,58E-02
GWP-b kg CO2 eqv. 3,45E-04 9,25E-06 6,51E-02 3,64E-06 0,00E+00 5,81E-07 -4,95E-04
GWP-f kg CO2 eqv. 2,05E-02 1,43E-02 1,78E-01 7,88E-03 0,00E+00 2,93E-04 8,63E-02
GWP-lu-
kg CO2 eqv.
luc 3,63E-05 8,35E-06 2,15E-04 2,89E-06 0,00E+00 8,16E-08 2,46E-05
ETP-fw CTUe 9,74E-01 1,88E-01 1,30E+00 1,06E-01 0,00E+00 5,31E-03 2,70E+00
disease inci-
PM
dence 1,00E-09 1,15E-09 2,07E-08 7,09E-10 0,00E+00 5,40E-11 7,64E-09
EP-m kg N eqv. 4,73E-05 3,38E-05 1,26E-04 1,61E-05 0,00E+00 9,56E-07 7,37E-05
EP-fw kg PO4 eqv. 1,45E-06 1,50E-07 5,83E-06 7,95E-08 0,00E+00 3,28E-09 4,14E-06
EP-T mol N eqv. 5,43E-04 3,72E-04 2,92E-03 1,78E-04 0,00E+00 1,05E-05 8,68E-04
HTP-c CTUh 9,68E-10 6,35E-12 2,21E-10 3,44E-12 0,00E+00 1,23E-13 5,19E-10
HTP-nc CTUh 2,29E-10 1,96E-10 1,23E-08 1,16E-10 0,00E+00 3,77E-12 5,35E-09
kBq U235
IR
eqv. 2,32E-03 8,88E-04 1,88E-02 4,98E-04 0,00E+00 3,36E-05 1,14E-03
SQP Pt 2,08E-01 1,80E-01 1,41E+00 1,03E-01 0,00E+00 1,72E-02 1,85E-01
kg CFC 11
ODP
eqv. 1,75E-09 3,06E-09 2,65E-08 1,74E-09 0,00E+00 1,21E-10 4,21E-09
kg NMVOC
POCP
eqv. 1,51E-04 1,04E-04 3,47E-04 5,07E-05 0,00E+00 3,06E-06 4,59E-04
ADP-f MJ 3,32E-01 2,11E-01 3,51E+00 1,19E-01 0,00E+00 8,19E-03 9,01E-01
ADP-mm kg Sb-eqv. 5,00E-07 3,26E-07 2,29E-06 2,00E-07 0,00E+00 2,68E-09 1,91E-08
m3 world
WDP
eqv. 7,01E-03 7,88E-04 5,69E-02 4,25E-04 0,00E+00 3,67E-04 5,38E-03
AP = Acidification; GWP-total = Global warming potential; GWP-b = Global warming potential – Biogenic; GWP-f = Global warming potential
– Fossil; GWP-luluc = Global warming potential - Land use and land use change; ETP-fw = Ecotoxicity, freshwater; PM = Particulate Matter;
EP-m = Eutrophication marine; EP-fw = Eutrophication, freshwater; EP-T = Eutrophication, terrestrial; HTP-c = Human toxicity, cancer; HTP-
nc = Human toxicity, non-cancer; IR = Ionising radiation, human health; SQP = Land use; ODP = Ozone depletion; POCP = Photochemical
ozone formation - human health; ADP-f = Resource use, fossils; ADP-mm = Resource use, minerals and metals; WDP = Water use
Table 11: Results of the LCA – Environmental parameters
Results of the LCA – Environmental parameters
Parameter Unit A1 A2 A3 C2 C3 C4 D
PERE MJ 1,04E-01 2,98E-03 2,16E+00 1,49E-03 0,00E+00 6,62E-05 2,03E-02
PERM MJ 0,00E+00 0,00E+00 1,14E-02 0,00E+00 0,00E+00 0,00E+00 0,00E+00
PERT MJ 1,04E-01 2,98E-03 2,17E+00 1,49E-03 0,00E+00 6,62E-05 2,03E-02
PENRE MJ 2,68E-01 2,24E-01 3,54E+00 1,26E-01 0,00E+00 8,69E-03 9,50E-01
PENRM MJ 8,26E-02 0,00E+00 2,03E-01 0,00E+00 0,00E+00 0,00E+00 0,00E+00
PENRT MJ 3,50E-01 2,24E-01 3,75E+00 1,26E-01 0,00E+00 8,69E-03 9,50E-01
SM kg 1,10E+00 0,00E+00 1,11E-03 0,00E+00 0,00E+00 0,00E+00 0,00E+00
RSF MJ 0,00E+00 0,00E+00 0,00E+00 0,00E+00 0,00E+00 0,00E+00 0,00E+00
NRSF MJ 0,00E+00 0,00E+00 0,00E+00 0,00E+00 0,00E+00 0,00E+00 0,00E+00
FW m3 2,84E-04 2,77E-05 2,10E-03 1,45E-05 0,00E+00 8,74E-06 1,61E-04
HWD kg 2,01E-07 5,36E-07 6,01E-07 3,01E-07 0,00E+00 1,22E-08 8,59E-06
NHWD kg 2,86E-02 1,18E-02 2,05E-02 7,54E-03 0,00E+00 5,56E-02 2,96E-03
RWD kg 2,00E-06 1,38E-06 2,04E-05 7,80E-07 0,00E+00 5,38E-08 1,28E-06
CRU kg 0,00E+00 0,00E+00 0,00E+00 0,00E+00 0,00E+00 0,00E+00 0,00E+00
MFR kg 0,00E+00 0,00E+00 3,68E-02 0,00E+00 1,06E+00 0,00E+00 0,00E+00
MER kg 0,00E+00 0,00E+00 0,00E+00 0,00E+00 0,00E+00 0,00E+00 0,00E+00
EET MJ 0,00E+00 0,00E+00 3,97E-03 0,00E+00 0,00E+00 0,00E+00 0,00E+00
EEE MJ 0,00E+00 0,00E+00 2,30E-03 0,00E+00 0,00E+00 0,00E+00 0,00E+00
PERE = Renewable primary energy ex. raw materials; PERM = Renewable primary energy used as raw materials; PERT = Renewable primary
energy total; PENRE = Non-renewable primary energy ex. raw materials; PENRM = Non-renewable primary energy used as raw materials;
PENRT = Non-renewable primary energy total; SM = Use of secondary material; RSF = use of renewable secondary fuels; NRSF = Use of
non-renewable secondary fuels; FW = Use of net fresh water; HWD = Hazardous waste disposed; NHWD = Non-hazardous waste disposed;
RWD = Radioactive waste disposed; CRU = Components for re-use; MFR = Materials for recycling; MER = Materials for energy recovery; EET
= Exported energy thermic; EEE = Exported energy electric
RIVA ACIER S.A.S. – EPD Hot Rolled concrete reinforcing bars | Seite 11
6. LCA: Interpretation
For an easier understanding, the results are processed graphically, in order to recognize relationships
and connections between the data more clearly.
The following figure shows the percentage of the product phases in the environmental impact cate-
gories.
WDP
ADP-mm
ADP-f
POCP
ODP
SQP
IR
HTP-nc
HTP-c
EP-T
EP-fw
EP-m
PM
ETP-fw
GWP-luluc
GWP-f
GWP-b
GWP-total
AP
-20% 0% 20% 40% 60% 80% 100%
A1 A2 A3 C2 C3 C4 D
Figure 1: Percentage of the product phases in the environmental impact categories
The figure shows that for the environmental impact categories raw material supply A1 during the pro-
duction phase and Reuse-Recovery-Recycling-potential module D have the highest percentages. The
high share of production phase A3 is related to the high electricity consumption in steelmaking with
an electric arc furnace (EAF). The high value for the impact category HTP-nc is related to the high share
of nuclear energy in electricity production.
RIVA ACIER S.A.S. – EPD Hot Rolled concrete reinforcing bars | Seite 12
7. References
Ecoinvent, 2019 Ecoinvent Datenbank Version 3.6 (2019)
EN 15804 EN 15804:2012+A2:2019: 2020: Sustainability of construction works - Environ-
mental product declarations - Core rules for the product category of construc-
tion products
ISO 14025 DIN EN ISO 14025:2011-10: Environmental labels and declarations — Type III
environmental declarations — Principles and procedures
ISO 14040 DIN EN ISO 14040:2006-10, Environmental management - Life cycle assess-
ment - Principles and framework; EN ISO 14040:2006
ISO 14044 DIN EN ISO 14044:2006-10, Environmental management - Life cycle assess-
ment - Requirements and guidelines; EN ISO 14040:2006
PCR A General Program Category Rules for Construction Products from the EPD pro-
gramme of Kiwa BCS Öko-Garantie GmbH - Ecobility Experts; Version 2.0
PCR B Product Category Rules for steel construction products from the EPD pro-
gramme of Kiwa BCS Öko-Garantie GmbH - Ecobility Experts; Requirements on
the Environmental Product Declarations for steel construction products; Ver-
sion 2020-03-13 (draft)
R<THiNK, 2021 R<THiNK; Online-EPD-Tool von Nibe; 2021
RIVA ACIER S.A.S. – EPD Hot Rolled concrete reinforcing bars | Seite 13
Publisher:
Kiwa GmbH – Ecobility Ex- Mail DE.Ecobility.Experts@kiwa.com
perts
Web https://www.kiwa.com/de/en/them
Voltastr. 5 es/ecobility-experts/
13355 Berlin
Germany
Programme operator:
Kiwa – Ecobility Experts Mail DE.Ecobility.Experts@kiwa.com
Voltastr. 5 Web https://www.kiwa.com/de/en/them
es/ecobility-experts/
13355 Berlin
Germany
Provider of the LCA:
Kiwa GmbH Tel +49 30 467761 43
Voltastr. 5 Fax +49 30 467761 10
13355 Berlin Mail Anna.Menegazzi@kiwa.com
Germany Web www.kiwa.com
Owner of the declaration:
RIVA ACIER S.A.S. Tel +33 1 30 98 20 00
Immeuble ALPA Web www.rivaacier.com
ZI Limay Porcheville Mail commercial.france@rivagroup.com
78440 Gargenville
France
RIVA ACIER S.A.S. – EPD Hot Rolled concrete reinforcing bars | Seite 14
