ENVIRONMENTAL PRODUCT DECLARATION
as per ISO 14025 and EN 15804+A2
Owner of the Declaration Armacell GmbH
Programme holder Institut Bauen und Umwelt e.V. (IBU)
Publisher Institut Bauen und Umwelt e.V. (IBU)
Declaration number EPD-ARM-20200222-IBA1-EN
Issue date 12.03.2021
Valid to 11.03.2026
HT/ArmaFlex insulation for building equipment and industrial
installations
Armacell GmbH
www.ibu-epd.com | https://epd-online.com
Umwelt Produktdeklaration Name des Herstellers – Name des Produkts
1. General Information
Armacell GmbH HT/ArmaFlex
Programme holder Owner of the declaration
IBU – Institut Bauen und Umwelt e.V. Armacell GmbH
Panoramastr. 1 Robert-Bosch-Str. 10
10178 Berlin 48153 Münster - Germany
Germany
Declaration number Declared product / declared unit
EPD-ARM-20200222-IBA1-EN 1m³ insulation material HT/ArmaFlex
This declaration is based on the product Scope:
category rules: Product line HT/ArmaFlex
Insulating materials made of foam plastics, 06.2017 Insulation material for industrial and building
(PCR checked and approved by the SVR) installations vulcanized in tubes and sheets.
This declaration is an Environmental Product
Issue date Declaration according to ISO 14025 describing the
12.03.2021 specific environmental performance of the product
produced in Germany.
Valid to As the installation of the product is not restricted to
countries where the products have been produced the
11.03.2026
validity of this EPD is considered at least EU wide.
The owner of the declaration shall be liable for the
underlying information and evidence; the IBU shall not
be liable with respect to manufacturer information, life
cycle assessment data and evidences.
The EPD was created according to the specifications
of EN 15804+A2. In the following, the standard will be
simplified as EN 15804.
Verification
The standard EN 15804 serves as the core PCR
Independent verification of the declaration and data
according to ISO 14025:2010
Dipl. Ing. Hans Peters internally x externally
(chairman of Institut Bauen und Umwelt e.V.)
Dr. Alexander Röder Mr Carl-Otto Neven
(Managing Director Institut Bauen und Umwelt e.V.)) (Independent verifier)
2. Product
2.1 Information about the enterprise The product focus is insulation materials enhancing the
Armacell International GmbH is a producer of flexible energy efficiency of technical equipment, high-
insulation foams for the equipment insulation market performance foams for technical and lightweight
and a provider of engineered foams which operates applications, 100% recycled PET products and next-
two main businesses: generation aerogel technology.
 Advanced Insulation develops flexible foams
for the insulation of technical equipment 2.2 Product description/Product definition
HT/ArmaFlex is the professional, highly-flexible,
utilised for the transport of energy - such as
closed-cell elastomeric foam insulation (FEF) for
heating, ventilation & air conditioning (HVAC)
continuous energy saving and condensation control
and heating & plumbing (H&P) in residential
purposes with exceptional resistance to high
and commercial construction, process lines in temperatures and UV radiation. The combination of
the heavy- and oil & gas industry, equipment very low thermal conductivity and extremely high
in transportation, as well as, acoustics. resistance to water vapour transmission prevents long-
term energy losses and water vapour ingress and
 Engineered Foams develops high-
reduces the risk of corrosion under insulation.
performance foams for the use in a broad
range of end markets including transportation,
automotive, wind energy, sports and For the placing on the market of the product in the
construction. European Union/European Free Trade Association
2 Environmental Product Declaration Armacell GmbH – HT/ArmaFlex insulation for industrial and building installation
(EU/EFTA) (with the exception of Switzerland) Name Value Unit
Regulation (EU) No. 305/2011 (CPR) applies. The Rubber and polymers 19 %
product needs a declaration of performance taking into Fillers and pigments 12 %
consideration EN 14304:2013-04 and the CE-marking. Blowing agent 7 %
For the application and use the respective national Vulcanisation system, additives,
33 %
provisions apply. plasticisers
Flame retardant 30 %
2.3 Application
HT/ArmaFlex is used to insulate pipes, air ducts and Synthetic rubber determines the flexibility;
vessels including fittings and flanges of industrial Fillers determine the fire properties and firmness;
installations and building equipment. Blowing agent causes the expansion process during
 Condensation control, energy saving and manufacturing;
noise control in refrigeration and air Accelerator and sulphur enable the vulcanisation;
conditioning equipment and process plants. Plasticizers determine the flexibility;
Flame retardants ensure fire resistance.
 Energy savings and personal protection
insulation in solar panels, hot gas lines, steam
According to the European Chemicals Regulation
and dual temperature lines applications.
REACH manufacturer, importers and downstream
users must register their chemicals and are
responsible for their safe use on their own. For its
2.4 Technical Data production Armacell uses exclusively verifiably
registered and approved substances / mixtures.
According to available data and the information
Constructional data provided by preliminary suppliers, the product does not
Name Value Unit contain substances (SVHC) that are considered
Gross density 75 kg/m3 substances meeting the criteria for inclusion in annex
Water vapour diffusion resistance XIV (List of Substances Subject to Authorisation) as
≥ 4000 / ≥
factor acc. to EN 12086, EN - laid down in Article 57 and article 59 of REACH (EC)
3000
13469 1907/2006.). Products manufactured and marketed by
0,042/0,04 Armacell do not have to be registered. The products
Thermal conductivity 5 (40°C) W/(mK) may contain traces of azodicarbonamide (ACDA).
Maximum service temperature Possible minimal residual amounts are included in the
acc. to EN 14706, EN 14707 +150 °C polymer matrix. A health impairment can be excluded.
For the production of insulation material based on
Minimum service temperature -50 °C
synthetic rubber, there is presently no alternative to
Tubes: DL-
ADCA available.
Reaction to fire acc. to EN 13501- s3, d0/
-
1 Sheets: D-
s3, d0
Structure-borne sound
not 2.7 Manufacture
transmission acc. to EN ISO
relevant ArmaFlex products are manufactured in a
3822-1
pressureless, continuous and discontinuous production
Weighted sound absorption
not process.
coefficient αw acc. to EN ISO
relevant In the first step, a homogenous compound is produced
11654
with rubber, additives, ancillary materials, blowing and
vulcanization agents. This is done on the rolling mill or
Insulation materials on the basis of synthetic rubber do
in the internal mixer followed by the rolling mill.
not absorb moisture from the air. For this reason the
Rubber extruders are used to process the compounds
normal building moisture does not lead to an increase
to produce raw profiles with defined dimensions. Here
in thermal conductivity.
exact compliance with the dimensions for the raw
profile is crucial for the dimensional accuracy of the
Performance data of the product in accordance with
foamed product.
the declaration of performance with respect to its
In the case of the discontinuous, pressureless
essential characteristics according to EN 14304:2013-
production process, the raw profiles are cut to length
04
and then foamed in a hot-air oven. In the case of the
continuous, pressureless process, the extruded profile
2.5 Delivery status
is fed directly onto a vulcanization line whose energy
FEF made of cross-linked elastomer is supplied as
source may be hot air, for example.
sheets, tubes and shaped pieces. Insulation
In foam production, vulcanization and blowing
thicknesses are available for all common pipe
processes run alongside each other. Both reactions
diameters up to an outer diameter of 89 mm (tubes).
are regulated by temperature control. Recipe and
temperature control determine the properties of the
2.6 Base materials/Ancillary materials
foam.
Quality assurance:
ArmaFlex is a highly flexible insulation material based
EC Certificate of conformity no. 0543 of the
on synthetic rubber, which consists of around 20 basic
Gütegemeinschaft Hartschaum e.V. Celle.
components. The following table displays the
Quality management system in accordance with EN
composition split into functional substance groups.
ISO 9001.
3 Environmental Product Declaration Armacell GmbH – HT/ArmaFlex insulation for industrial and building installation
2.8 Environment and health during
manufacturing 2.14 Extraordinary effects
During all manufacturing steps and at all production
sites of Armacell, the production follows the national Fire
guidelines and regulations. A regenerative thermal According to EN 13501, ArmaFlex is classified as a
oxidizer is installed to treat exhaust air. combustible insulation material. Due to its material
Certification of the environmental management system structure ArmaFlex does not contribute to an
is in accordance with ISO 14001. uncontrollable spread of fire under installation
conditions typical on a building site. ArmaFlex does not
drip under practical fire conditions, this means that fire
2.9 Product processing/Installation spread is ruled out. The product is self-extinguishing
The product is installed by using knives. No special and therefore only makes a minor contribution to the
tools, nor specific protection is necessary. actual fire event. There is no possibility of the material
When applying adhesives the information given in the self-igniting. ArmaFlex does not propagate the fire
relevant safety data sheets is to be heeded. either horizontally or vertically.
The recommendations for installing the product
depend on the product and system and are described Fire protection
in the respective documents (e.g. Armaflex application Name Value
manual) and on the data sheets. More details under Tubes: DL
www.armacell.com. Euro class / Sheets:
D
Tubes/She
Burning droplets
2.10 Packaging ets: d0
As a rule, ArmaFlex products are packaged in Tubes/She
Smoke development
cardboard boxes and transported on reusable pallets. ets: s3
Over-sized rolls of sheet material are packaged in
polyethylene (PE) foil. The cardboard boxes can be Water
recycled through Interseroh’s dual system. Armacell insulation materials have a high resistance to
water vapour transmission which keeps possible water
vapour transmission processes to a minimum
2.11 Condition of use permanently. Therefore, a significant reduction in the
When the products are used for the purpose for which insulation effect can be ruled out permanently.
they are intended, there are no changes in the material If the insulation material is exposed to water over a
composition during use, except in the event of long period of time (e.g. flooding) it should be replaced.
extraordinary impacts (see 2.14).
Mechanical destruction
2.12 Environment and health during use ArmaFlex insulation materials are flexible foams and
Ingredients: There are no particular aspects of the thus display limited mechanical stability. Therefore, if
material composition during use. the material will be subject to greater mechanical
Eurofins Product Testing A/S has tested a wide range impact it should be protected appropriately, e.g. by a
and varieties of typical FEF (Flexible Elastomeric metal jacket or Arma-Chek covering.
Foam) products marketed in the EU from CEFEP ArmaFlex products (with the exception of
(European Group of FEF manufacturers). Sampling, HT/ArmaFlex) are not UV resistant. If the material is
testing and evaluation were performed according to subject to UV-rays it should be protected accordingly.
CEN TS 16516, AgBB, ISO 16000-3, ISO 16000-6,
ISO 16000-9, ISO 16000-11 in the latest versions.
Based on the loading factor 0.05 m²/m³, which was 2.15 Re-use phase
determined after consideration of real life applications If removed properly the product can be re-used.
with FEF products (in living rooms) and Correctly sorted material can be ground and used to
recommendation of experts of the test institute, all manufacture new products (e.g. ArmaSound).
results were clearly below the limit values. For
example, the determined total volatile organic 2.16 Disposal
compound (TVOC) after 28 days was for all samples Dispose of the materials according to local regulations.
below 100 mg/m3. Certificates are available on Regulated by the European Waste Catalogue: Waste
request. code 07 02 13 (waste plastic).
Note: Please observe Commission Decision
2001/118/EC.
2.13 Reference service life
ArmaFlex products are long-lasting products. Findings 2.17 Further information
show that when used and installed properly they can Further information on ArmaFlex® can be found on the
have an estimated service life of more than 50 years. It manufacturer’s website www.armacell.com. Detailed
is practically only restricted by the service life of the specification clauses for the products are provided at
equipment or whole building, which can extent that www.armaflex.de.
time period.. The insulation performance is almost
completely maintained over the entire service life. The
insulation performance is only compromised by
extraordinary impacts and damage during construction.
4 Environmental Product Declaration Armacell GmbH – HT/ArmaFlex insulation for industrial and building installation
3. LCA: Calculation rules
3.1 Declared Unit End-of-life (C2, C3):
The declaration refers to 1 m³ insulation product. The transport from place of usage to a waste
For the LCA calculations the average density per incineration plant is assumed as 100 km.
product brand is used. After the demolition of the product a current realistic
As additional information and support for installers the End-of-life scenario is the incineration of the material.
thermal conductivity coefficient (lambda-value) and R- According to the reported net calorific value of the
value per 20 cm thickness per product brand are given. materials and the elementary composition, a partial
stream consideration for the incineration process of
Declared unit PVC-products is applied as an approximation for all
Name Value Unit declared products.
Declared unit 1 m3 Inventory estimations and approximations:
Gross density 75 kg/m3 The reported recipes for the rubber mixes contain
Conversion factor to 1 kg 75 - specific substances of the rubber industry. For these
materials only partly life cycle inventories are available.
Thermal conductivity λ : 0.045 W/(mK (0°C) Approximations are used with the consideration of
R-value – thickness: 20 cm: 4.4 (m²K)/W similar supply chain effort or similar elementary
composition. Partly an estimation is modelled using
pre-products of the specific material and adding an
energy effort as well as considering the treatment of
3.2 System boundary production residues for this step in the supply chain.
The data collection refers to the yearly production in
2019. The following life cycle stages are considered. 3.4 Cut-off criteria
In the assessment, all reported data from the
Type of EPD: Cradle-to-Gate with options: production process are considered, utilised thermal
energy, and electric power consumption using best
Production A1-A3: available life cycle inventory (LCI) datasets. Thus
The LCA calculation covers the production of the raw material and energy flows contributing less than 1% of
materials (supply chain – A1), the mixing of raw mass or energy are considered.
materials according to the respective recipes No cut-off criteria are applied in the foreground data in
(MasterBatch) exclusively done in Münster, Germany, this study.
the transport (A2) of the MasterBatches to the For cut-off criteria in the background system, see
production facility for foaming and the foaming process information provided in the modelling principles and
(A3) in Germany, Spain, Poland or Great Britain, specific documentations (documentation.gabi-
including the packaging material. software.com).
Transport A4:
Average values for the transport from factory gate to 3.5 Background data
construction site are assumed. The LCA model is created using the GaBi ts Software
Installation A5: system (v9) for life cycle engineering, developed by
The installation considers the production of off-cuts, Sphera. The GaBi LCI database provides the life cycle
incineration of these off-cuts and the disposal scenario inventory data for several of the raw and process
for the packaging material. Auxiliaries like adhesives or materials obtained from the background system. The
tapes or energy for installation are not considered. most recent update of the database was 2020.
End-of-life C2, C3:
An incineration scenario for the used and demolished 3.6 Data quality
product, including an assumption for the transport to The foreground data collected by the manufacturer are
disposal, is covered. based on yearly production amounts and
Benefits for the next product system D: extrapolations of measurements on specific machines
Credits for electrical and thermal energy resulting from and plants.
the waste incineration process of the off-cut material Most of the necessary life cycle inventories for the
and packaging (A5) and the product (C3) are declared basic materials are available in the GaBi database.
in module D. The last update of the database was in 2020 (service
pack 40).
Further LCIs for materials of the supply chain of the
3.3 Estimates and assumptions basic materials are approximated with LCIs of similar
Scenario assumptions: materials or estimated by the combination of available
Installation (A5): LCIs.
The additional demand of material for installation For electrical and thermal energy regional specific grid
depends on the specific frame conditions of the mixes and regional specific supply for natural gas are
building and pipe system to be insulated. Parts of the considered.
product can be joined; thus installation off-cut is very
small. A loss of 1% is assumed. 3.7 Period under review
Transport to customer (A4): The production data refer to an average of the year
Armacell’s data collectors reported average figures for 2019.
the distribution of their material. Depending on the
country, the transport distance varies from 500 km to 3.8 Allocation
800 km Allocation of upstream data:
5 Environmental Product Declaration Armacell GmbH – HT/ArmaFlex insulation for industrial and building installation
For all refinery products, allocation by mass and net Environmental burden of the incineration of installation
calorific value is applied. The specific manufacturing residues (off-cuts), packaging and the product in the
route of every refinery product is modelled and so the end-of-life scenario are assigned to the system (A5 or
impacts associated with the production of these C3); resulting credits for thermal and electrical energy
products are calculated individually. are declared in module D.
Materials and chemicals used in the manufacturing The credits for thermal and electrical energy are
process are modelled using the allocation rule most calculated via inversion of the life cycle inventory of
suitable for the respective product. For further European average data.
information on a specific product see Allocation for waste paper:
documentation.gabi-software.com. Paper/corrugated board is used as packaging material
Allocation in the foreground data: and this usually includes a mix of recycled and virgin
Part of the production residues (ca. 2%) are used for fibres. When modelling the production of paper, the
the manufacturing of a non-declared product scrap paper that is used in this process has been
(ArmaSound). These materials leave the process assumed to be burden free. Similarly, waste paper
without further consideration of any treatment and arising in the product life cycle is assumed to be
without credit (cut-off-approach). recycled. Robust data on paper and cardboard
No further allocation is applied in the software model. recycling are not promptly available and refer to a very
The overall production of the Armacell production complex system. Hence, to apply this methodology
facilities comprises further products beside the consistently throughout the model, a cut-off approach
products considered in this study. Data for thermal and has been applied, i.e., input of waste paper is
electrical energy, as well as auxiliary material, refer to considered without environmental burden, resulting
the declared products only. During data collection the waste paper is not credited. The recycling process and
allocation is done via mass, area, pieces or time spent the production process of paper are merged in the
in the machine, depending on the process step and production process. The C-balance referring to fresh
reasonable split. The data collectors at Armacell fibre is corrected via CO2 emissions (biotic)
decided on the distribution basis. (assumption of final rotting or incineration in the time
Allocation for waste materials: frame of 100 years).
Production waste is sent to a waste incineration plant
and to landfill (Spain). Resulting electrical and thermal 3.9 Comparability
energy from the incineration process is looped inside Basically, a comparison or an evaluation of EPD data
module A1-A3. The quality of the recovered energy is is only possible if all the data sets to be compared
assumed to the same as that of the input energy. were created according to EN 15804 and the building
Landfilling of plastic material is assumed not to deliver context, respectively the product-specific
any landfill gas. characteristics of performance, are taken into account.
All applied incineration processes are displayed via a
partial stream consideration for the combustion The used background dataset DB has been GaBi
process, according to the specific composition of the (service pack. 40, 2020).
incinerated material. For the waste incineration plant
an R1-value of > 0.6 is assumed.
4. LCA: Scenarios and additional technical information
Characteristic product properties Transport to the building site (A4)
Information on biogenic Carbon Name Value Unit
The biogenic carbon content quantifies the amount of Litres of fuel 0.22 l/100km
biogenic carbon in a construction product leaving the Transport distance 800 km
factory gate, and it shall be separately declared for the Capacity utilisation (including empty
85 %
product and for any accompanying packaging. runs)
If the total mass of biogenic carbon containing
materials is less than 5 % of the total mass of the Installation into the building (A5)
product and accompanying packaging, the declaration Name Value Unit
of biogenic carbon content may be omitted. The mass Material loss 1 %
of packaging containing biogenic carbon shall always
be declared.
Note: 1 kg biogenic Carbon is equivalent to 44/12 kg of
CO 2 Estimated service life
Information on describing the biogenic Carbon Name Value Unit
Content at factory gate Life Span according to the
50 a
Name Value Unit manufacturer
Biogenic Carbon Content in
0 kg C
product End of life (C1-C4)
Biogenic Carbon Content in Name Value Unit
27.24 kg C
accompanying packaging Energy recovery in WIP 75 kg
The embodied biogenic carbon leaves the system in
Module A5 Reuse, recovery and/or recycling potentials (D),
relevant scenario information
The following technical information serves as basis for Module D includes the credits of the incineration
the declared modules. The values refer to the declared processes from A5 (off-cut of product installation,
unit of 1 m³. packaging waste) and C3 (incineration of the product).
6 Environmental Product Declaration Armacell GmbH – HT/ArmaFlex insulation for industrial and building installation
A waste incineration plant with an R1-value > 0.6 is
assumed.
7 Environmental Product Declaration Armacell GmbH – HT/ArmaFlex insulation for industrial and building installation
5. LCA: Results
The following information on environmental impacts is expressed with the impact category parameters of LCIA
using characterisation factors. The chosen characterisation factors fulfil the requirements of EN 15804.
Disclaimer:
EP-freshwater: This indicator has been calculated as “kg P eq” as required in the characterization model
(EUTREND model, Struijs et al., 2009b, as implemented in ReCiPe;
http://eplca.jrc.ec.europa.eu/LCDN/developerEF.xhtml)
DESCRIPTION OF THE SYSTEM BOUNDARY (X = INCLUDED IN LCA; ND = MODULE OR INDICATOR NOT
DECLARED; MNR = MODULE NOT RELEVANT)
BENEFITS AND
CONSTRUCTI LOADS
PRODUCT STAGE ON PROCESS USE STAGE END OF LIFE STAGE BEYOND THE
STAGE SYSTEM
BOUNDARIES
8 Environmental Product Declaration Armacell GmbH – HT/ArmaFlex insulation for industrial and building installation
lairetam
waR
ylppus tropsnarT
gnirutcafunaM
eht
morf
tropsnarT
etis
eht
ot
etag
ylbmessA esU
ecnanetniaM
riapeR
tnemecalpeR tnemhsibrufeR
ygrene
lanoitarepO esu
retaw
lanoitarepO esu
noitcurtsnoc-eD
noitilomed tropsnarT
gnissecorp
etsaW
lasopsiD -esueR -yrevoceR -gnilcyceR laitnetop
A1 A2 A3 A4 A5 B1 B2 B3 B4 B5 B6 B7 C1 C2 C3 C4 D
X X X X X ND ND MNR MNR MNR ND ND ND X X ND X
RESULTS OF THE LCA - ENVIRONMENTAL IMPACT according to EN 15804+A2: 1 m³ HT/ArmaFlex
insulation for industrial and building installation
Core Indicator Unit A1-A3 A4 A5 C2 C3 D
Global warming potential - total [kg CO2-Eq.] 2.18E+2 5.33E+0 1.10E+2 3.58E-1 1.95E+2 -5.40E+1
Global warming potential - fossil fuels [kg CO2-Eq.] 3.19E+2 5.30E+0 6.06E+0 3.56E-1 1.95E+2 -5.39E+1
Global warming potential - biogenic [kg CO2-Eq.] -1.02E+2 -9.04E-3 1.04E+2 -6.07E-4 -8.50E-2 -1.26E-1
GWP from land use and land use change [kg CO2-Eq.] 8.77E-1 4.29E-2 9.89E-3 2.88E-3 3.96E-2 -3.76E-2
Depletion potential of the stratospheric ozone layer [kg CFC11-Eq.] 7.76E-10 6.37E-16 7.84E-12 4.27E-17 2.96E-13 -5.60E-13
Acidification potential, accumulated exceedance [mol H+-Eq.] 2.41E+0 1.59E-2 2.80E-2 1.07E-3 5.78E-2 -7.53E-2
Eutrophication, fraction of nutrients reaching freshwater
end compartment
[kg PO4-Eq.] 2.96E-3 1.61E-5 3.09E-5 1.08E-6 4.99E-5 -6.92E-5
Eutrophication, fraction of nutrients reaching marine end
[kg N-Eq.] 2.13E-1 7.07E-3 3.34E-3 4.75E-4 1.91E-2 -1.95E-2
compartment
Eutrophication, accumulated exceedance [mol N-Eq.] 2.22E+0 7.92E-2 3.90E-2 5.32E-3 2.34E-1 -2.09E-1
Formation potential of tropospheric ozone photochemical
[kg NMVOC-Eq.] 9.41E-1 1.40E-2 1.27E-2 9.38E-4 5.42E-2 -5.60E-2
oxidants
Abiotic depletion potential for non-fossil resources [kg Sb-Eq.] 5.46E+3 7.05E+1 6.39E+1 4.73E+0 3.59E+2 -9.13E+2
Abiotic depletion potential for fossil resources [MJ] 2.72E+0 3.80E-7 2.75E-2 2.55E-8 4.26E-6 -8.82E-6
Water (user) deprivation potential, deprivation-weighted [m³ world-Eq
2.67E+1 4.73E-2 2.48E+0 3.18E-3 1.50E+1 -5.56E+0
water consumption (WDP) deprived]
RESULTS OF THE LCA - INDICATORS TO DESCRIBE RESOURCE USE according to EN 15804+A2: 1 m³
HT/ArmaFlex insulation for industrial and building installation
Indicator Unit A1-A3 A4 A5 C2 C3 D
Renewable primary energy as energy carrier [MJ] 1.97E+3 3.96E+0 1.62E+2 2.66E-1 7.44E+1 -1.99E+2
Renewable primary energy resources as material utilization [MJ] 1.39E+2 0.00E+0 -1.39E+2 0.00E+0 0.00E+0 0.00E+0
Total use of renewable primary energy resources [MJ] 2.11E+3 3.96E+0 2.29E+1 2.66E-1 7.44E+1 -1.99E+2
Non-renewable primary energy as energy carrier [MJ] 4.10E+3 7.06E+1 7.32E+1 4.74E+0 1.73E+3 -9.14E+2
Non-renewable primary energy as material utilization [MJ] 1.38E+3 0.00E+0 -9.23E+0 0.00E+0 -1.37E+3 0.00E+0
Total use of non-renewable primary energy resources [MJ] 5.48E+3 7.06E+1 6.40E+1 4.74E+0 3.59E+2 -9.14E+2
Use of secondary material [kg] 3.87E+1 0.00E+0 0.00E+0 0.00E+0 0.00E+0 0.00E+0
Use of renewable secondary fuels [MJ] 0.00E+0 0.00E+0 0.00E+0 0.00E+0 0.00E+0 0.00E+0
Use of non-renewable secondary fuels [MJ] 0.00E+0 0.00E+0 0.00E+0 0.00E+0 0.00E+0 0.00E+0
Use of net fresh water [m³] 1.80E+0 4.59E-3 7.06E-2 3.08E-4 3.95E-1 -2.30E-1
RESULTS OF THE LCA – WASTE CATEGORIES AND OUTPUT FLOWS according to EN 15804+A2:
1 m³ HT/ArmaFlex insulation for industrial and building installation
Indicator Unit A1-A3 A4 A5 C2 C3 D
Hazardous waste disposed [kg] 4.05E-5 3.28E-6 4.62E-7 2.21E-7 1.62E-6 -3.64E-7
Non-hazardous waste disposed [kg] 2.66E+1 1.08E-2 1.65E+0 7.25E-4 1.19E+2 -4.21E-1
Radioactive waste disposed [kg] 1.18E-1 8.74E-5 1.55E-3 5.86E-6 1.14E-2 -6.79E-2
Components for re-use [kg] 0.00E+0 0.00E+0 0.00E+0 0.00E+0 0.00E+0 0.00E+0
Materials for recycling [kg] 0.00E+0 0.00E+0 5.44E+1 0.00E+0 0.00E+0 0.00E+0
Materials for energy recovery [kg] 0.00E+0 0.00E+0 0.00E+0 0.00E+0 0.00E+0 0.00E+0
Exported electrical energy [MJ] 0.00E+0 0.00E+0 2.91E+1 0.00E+0 1.96E+2 0.00E+0
Exported thermal energy [MJ] 0.00E+0 0.00E+0 5.23E+1 0.00E+0 3.57E+2 0.00E+0
RESULTS OF THE LCA – additional impact categories according to EN 15804+A2-optional:
1 m³ HT/ArmaFlex insulation for industrial and building installation
Indicator Unit A1-A3 A4 A5 C2 C3 D
Potential incidence of disease due to PM emissions [Disease
1.57E-4 8.79E-8 1.61E-6 5.90E-9 1.39E-6 -6.39E-7
Incidence]
Potential Human exposure efficiency relative to U235 [kBq U235-
1.31E+1 1.26E-2 1.82E-1 8.48E-4 1.16E+0 -1.11E+1
Eq.]
Potential comparative toxic unit for ecosystems [CTUe] 6.19E+3 4.98E+1 6.80E+1 3.35E+0 2.98E+2 -1.96E+2
Potential comparative toxic unit for humans - cancerogenic [CTUh] 1.45E-7 1.04E-9 1.72E-9 7.01E-11 1.18E-8 -8.53E-9
Potential comparative toxic unit for humans - not cancerogenic [CTUh] 2.21E-5 6.07E-8 2.41E-7 4.07E-9 1.25E-6 -3.17E-7
Potential soil quality index [-] 6.62E+3 2.47E+1 6.92E+1 1.66E+0 8.14E+1 -1.43E+2
Disclaimer 1 – for the indicator IRP
This impact category deals mainly with the eventual impact of low dose ionizingradiation on human health of the
nuclear fuel cycle. It does not consider effects due to possiblenuclear accidents, occupational exposure nor due to
radioactive waste disposal in undergroundfacilities. Potential ionizing radiation from the soil, from radon and some
construction materials is also not measured by this indicator.
Disclaimer 2 – for the indicators ADPE, ADPF, WDP, ETP-fw, HTP-c, HTP-nc, SQP
The results of this environmental impact indicator shall be used with care as theuncertainties on these results are
high or as there is limited experience with the indicator.
6. LCA: Interpretation
The supply chain, i.e. the production of the purchased the overall green house gas emissions. At the same
materials, causes the highest influence on all impact time a credit (D) of 11% is given to the next system,
categories and the primary energy. due to the use of electrical and thermal energy, gained
in the incineration processes for the product and the
Global Warming Potential off-cut material.
Looking at the GWP for the overall declared life cycle
phases, including production (A1-A3), transport (A4, Further impact categories
C2), installation (losses) (A5) and end-of-life (C3, D), The end-of-life scenarios have less influence on the
the production (A1-A3) contributes to 46%. other considered impact categories than on GWP. The
The production in the supply chain (A1) already main contribution of the considered life cycle phases is
contributes 42% to the total GWP value. Thus, every concentrated on module A1-A3.
increase in production yield directly improves the The energy consumption in the foaming step
environmental performance of the products. influences all impact categories; variations depend on
The foaming process (A3), which includes the the national grid mixes for electricity.
electrical and thermal energy for the mixing, the
vulcanisation and blowing step as well as the Primary Energy Demand
production of the packaging materials, shows a The total primary energy demand is for both categories
significant influence on GWP of the life cycle with 4%. (renewable and non-renewable) significantly (> 100%)
Module A5 covers the production and disposal influenced by the production of the module A1-A3. The
(=incineration) of the off-cut material assumed as 1% other modules play a minor role (C3 with about 6%)
loss in respect to the required insulation material.
Additionally, the emissions of the incineration of The share of primary energy bound as material
packaging material (plastic, wood) in a waste accounts for about 21%, which is partly recovered and
incineration plant are considered. The installation step credited for in module D (-16%)
contributes with 23% to the overall GWP.
As end-of-life scenario an incineration is considered.
The emissions of the product (C3) contribute to 41% to
7. Requisite evidence
recommendation of the experts of the test institute, all
7.1 VOC emissions results were clearly below the limit values. For
Eurofins Product Testing A/S has tested a wide range example the determined total volatile organic
and varieties of typical FEF (Flexible Elastomeric compound (TVOC) after 28 days was for all samples
Foam) products marketed in the EU from CEFEP below 100 mg/m3. Certificates are available on
(European Group of FEF manufacturers). Sampling, request.
testing and evaluation were performed according to
CEN TS 16516, AgBB, ISO 16000-3, ISO 16000-6, 7.2 Leaching performance
ISO 16000-9, ISO 16000-11 in the latest versions. According to EN 13468 is the content of water-soluble
Based on the loading factor 0.05 m²/m³, which were chloride ions for HT/Armaflex ≤ 80 ppm.
determined after consideration of real life applications
with FEF products (in living rooms) and
9 Environmental Product Declaration Armacell GmbH – HT/ArmaFlex insulation for industrial and building installation
8. References
AgBB building equipment and industrial installations -
Umweltbundesamt Germany, Health-related Determination of maximum service temperature
Evaluation of Emissions of Volatile Organic
Compounds (VVOC, VOC and SVOC) from Building EN 14707
Products EN 14707: 2013-01: Thermal insulating products for
building equipment and industrial installations -
CEFEP Determination of maximum service temperature for
The industry association for FEF and PEF insulation preformed pipe insulation
(Celle) in 2012
EN 15801
CEN TS 16516 EN 15801: 2010-04: Conservation of cultural property -
CEN TS 16516:2013-12: Construction products - Test methods - Determination of water absorption by
Assessment of release of dangerous substances - capillarity
Determination of emissions into indoor air
EN 15804
Comission Decision 2001/118/EC EN 15804:2012-04+A1 2013, Sustainability of
Amendment to European Waste Catalogue construction works — Environmental Product
Declarations — Core rules for the product category of
CPR construction products.
Regulation (EC) No 305/2011, Construction Products
Regulation EN 15804
EN 15804:2019+A2 (in press), Sustainability of
EN 826 construction works — Environmental Product
EN 826: 2013-05: Thermal insulating products for Declarations — Core rules for the product category of
building applications - Determination of compression construction products.
behaviour
EN 29052
EN 1606 EN 29052: 1992-08: Acoustics; determination of
EN 1606: 2013-05: Thermal insulating products for dynamic stiffness; part 1: materials used under floating
building applications - Determination of compressive floors in dwellings
creep
EU/EFTA
EN 12091 Regulation (EU) No. 305/2011 (CPR), European
EN 12091: 2013-06: Thermal insulating products for Union/European Free Trade Association (EU/EFTA)
building applications - Determination of freeze-thaw
resistance Eurofins Product Testing A/S
Eurofins Miljo, Smedeskowej 38, 8464 Galten,
EN 12086 Denmark
EN 12086:2013-06: Thermal insulating products for
building applications - Determination of water vapour European Waste Catalogue
transmission properties European Waste Catalogue and Hazardous Waste
List, Commission Decision 2000/532/EC
EN 13468
EN 13468: 2001-12: Thermal insulating products for GaBi
building equipment and industrial installations - GaBi 9 software-system and databases, LBP,
Determination of trace quantities of water soluble University of Stuttgart and Sphera, Leinfelden-
chloride, fluoride, silicate, and sodium ions and pH Echterdingen, 2020 (http://documentation.gabi-
software.com/)
EN 13469
EN 13469:2013-01: Thermal insulating products for IBU
building equipment and industrial installations - Institut Bauen und Umwelt e.V.: General Programme
Determination of water vapour transmission properties Instructions for the Preparation of EPDs at the Institut
of preformed pipe insulation Bauen und Umwelt e.V. Version 1., Berlin: Institut
Bauen und Umwelt e.V., 2016. www.ibu-epd.com
EN 13501-1
EN 13501-1: 2010-01: Fire classification of IBU PCR Part A
construction products and building elements - Part 1: PCR - Part A: Calculation Rules for the Life Cycle
Classification using data from reaction to fire tests Assessment and Requirements on the Project Report,
Institut Bauen und Umwelt e.V., www.ibu-epd.com,
EN 14304 2019.
EN 14304:2013-04: Thermal insulation products for
building equipment and industrial installations – IBU PCR PART B
Factory made flexible elastomeric foam (FEF) products PCR – Part B: Requirements on the EPD for Insulation
– Specification materials made of foam plastics, version 1.7, 01-2019 ,
Institut Bauen und Umwelt e.V., www.ibu-epd.com,
EN 14706 2019
EN 14706: 2013-01: Thermal insulating products for
10 Environmental Product Declaration Armacell GmbH – HT/ArmaFlex insulation for industrial and building installation
ISO 3822-1 Determination of the emission of volatile organic
ISO 3822-1: 1999-05: Acoustics - Laboratory tests on compounds from building products and furnishing -
noise emission from appliances and equipment used in Sampling, storage of samples and preparation of test
water supply installations - Part 1: Method of specimens
measurement
ISO 16000-3
ISO 9001 ISO 16000-3:2011-10: Determination of formaldehyde
ISO 9001:2014-08: Quality management systems – and other carbonyl compounds in indoor air and test
Requirements chamber air - Active sampling method
ISO 11654 ISO 16000-6
ISO 11654: 1997-04: Acoustics - Sound absorbers for ISO 16000-6:2011-12: Indoor air - Part 6:
use in buildings - Rating of sound absorption Determination of volatile organic compounds in indoor
and test chamber air by active sampling on Tenax TA®
ISO 14001 sorbent, thermal desorption and gas chromatography
ISO 14001:2015, Environmental management systems using MS or MS-FID
— Requirements with guidance for use
ISO 16000-9
ISO 14025 ISO 16000-9:2006-02: Indoor air - Part 9:
ISO 14025:2011-10, Environmental labels and Determination of the emission of volatile organic
declarations — Type III environmental declarations — compounds from building products and furnishing -
Principles and procedures. Emission test chamber method
ISO 14040
ISO 14040:2009-11: Environmental management – REACH
Life cycle assessment – Principles and framework Regulation (EC) No 1907/2006, Regulation concerning
the Registration, Evaluation, Authorisation and
ISO 14044 Restriction of Chemicals (REACH)
ISO 14044:2006-10: Environmental management –
Life cycle assessment – Requirements and guidelines
ISO 15868
ISO 15686:2011-05, Buildings and constructed assets
- Service life planning
ISO 16000-11
ISO 16000-11: 2006-02: Indoor air - Part 11:
11 Environmental Product Declaration Armacell GmbH – HT/ArmaFlex insulation for industrial and building installation
Publisher
Institut Bauen und Umwelt e.V. Tel +49 (0)30 3087748- 0
Panoramastr. 1 Fax +49 (0)30 3087748- 29
10178 Berlin Mail info@ibu-epd.com
Germany Web www.ibu-epd.com
Programme holder
Institut Bauen und Umwelt e.V. Tel +49 (0)30 - 3087748- 0
Panoramastr 1 Fax +49 (0)30 – 3087748 - 29
10178 Berlin Mail info@ibu-epd.com
Germany Web www.ibu-epd.com
Author of the Life Cycle
Assessment Tel +49 711 341817-0
Sphera Solutions GmbH Fax +49 711 341817-25
Hauptstraße 111- 113 Mail info@sphera.com
70771 Leinfelden-Echterdingen Web http://www.sphera.com
Germany
Owner of the Declaration
Armacell GmbH Tel +49-251-7603-0
Robert-Bosch-Str. 10 Fax +49-251-7603-346
48153 Münster Mail info.de@armacell.com
Germany Web www.armacell.de
