ENVIRONMENTAL PRODUCT DECLARATION
as per ISO 14025 and EN 15804+A2
Owner of the Declaration Hilti Aktiengesellschaft
Publisher Institut Bauen und Umwelt e.V. (IBU)
Programme holder Institut Bauen und Umwelt e.V. (IBU)
Declaration number EPD-HIL-20230140-IBA1-EN
Issue date 28/06/2023
Valid to 27/06/2028
HUS4-MAX and KHC
Hilti AG
www.ibu-epd.com | https://epd-online.com
1. General Information
Hilti AG HUS4-MAX and KHC
Programme holder Owner of the declaration
IBU – Institut Bauen und Umwelt e.V. Hilti Aktiengesellschaft
Hegelplatz 1 Feldkircher Strasse 100
10117 Berlin 9494 Schaan
Germany Liechtenstein
Declaration number Declared product / declared unit
EPD-HIL-20230140-IBA1-EN The
declared products are HILTI's HUS4-MAX and KHC adhesive capsules.
The declared unit is one kilogram of reaction resin product in the mixing
ratio of the two components necessary for processing. The packaging is
also included in the calculation. The declared unit is stated in [kg].
This declaration is based on the product category rules: Scope:
Reaction resin products, 01/08/2021 This document refers to the adhesive capsules HUS4-MAX and KHC with
(PCR checked and approved by the SVR) their packaging. For the compilation of the life cycle assessment, specific
data were collected from the factory in Kaufering, Germany, of the HILTI
AG. For the compilation of the life
Issue date cycle assessment, specific data were collected from the factory in
Kaufering, Germany, of the HILTI AG. Data from the years 2018 to 2021
28/06/2023
are used, which correspond to the annual average.
The owner of the declaration shall be liable for the underlying information
and evidence; the IBU shall not be liable with respect to manufacturer
Valid to
information, life cycle assessment data and evidences.
27/06/2028
The EPD was created according to the specifications of EN 15804+A2. In
the following, the standard will be simplified as EN 15804.
Verification
The standard EN 15804 serves as the core PCR
Independent verification of the declaration and data according to ISO
14025:2011
internally X externally
Dipl.-Ing. Hans Peters
(Chairman of Institut Bauen und Umwelt e.V.)
Dipl.-Ing. Hans Peters Matthias Klingler,
(Managing Director Institut Bauen und Umwelt e.V.) (Independent verifier)
1 Environmental-Product Declaration - Hilti AG - HUS4-MAX and KHC
2. Product
Name Value Unit
2.1 Product description/Product definition
Density (calculated value of uncured mortar (@
The declared products of HUS4-MAX and KHC adhesive 1124 kg/m3
20° )
capsules are two-component construction adhesives used in
Compressive strength (@23° C / 50 %
combination with mechanical screw anchors in Hilti's HUS4- 90.5 N/mm^2
humidity) acc. to EN ISO 604
MAX and Kwik-X Dual Anchor Action systems. Component A
comprises a resin based on methacrylate as well as mineral Compressive modulus (@23° C / 50 % humidity
1240 N/mm^2
filler. Component B comprises peroxide hardener, water and acc. to EN ISO 604
mineral filler. Hilti HUS4-MAX / KHC display the following characteristics:
During the setting of a mechanical screw anchor in a borehole
containing the adhesive capsule, the capsule foil is pierced to Performance data of the product in accordance with the
allow mixing of the two individual components which declaration of performance with respect to its essential
subsequently enables the A component to polymerase via characteristics according to
radicals released by the B component in a so-called chain
reaction. As a result a homogeneously cured mortar with ETA 18/1160
excellent proven mechanical properties, durability and bond ICC ESR-5065
strength arises over a very short curing time.
Composite foils are used for the HUS4-MAX and the KHC Shelf life:
capsules. This kind of packaging serves the following purposes: 18 months
waste volume reduction, easy storage and transport, less Substrate temperature at installation:
packaging material. +5° C to +40° C / +41° F to 104° F
The reaction resins used in Hilti adhesive capsules contain no
styrene, are practically odourless and have a considerably Curing time (base material temperature
higher flash point, i.e. higher than 100° C. For the placing of the at installation):
product on the market in the European Union European Free -28° C to -10° C / -18° F to +14° F 24 h
Trade Association EU/EFTA) (with the exception of Switzerland) > -10° C to +5° C / > 14° F to +41° F 30 min
the Regulation (EU) No. 305/2011 (CPR) applies. The product > +5° C to +40° C / > +41° F to +104° F 0.5 min
needs a declaration of performance taking into consideration
the following European Technical Approval 2.4 Delivery status
The product Hilti HUS4-MAX is available in M10, M12, M14 and
ETA 18/1160 M16 foil capsules.
The product Hilti KHC is available in 3/8" SMALL, 3/8" LARGE,
and the CE marking. For the application and use the respective 1/2" SMALL, 1/2" LARGE, 3/4" SMALL, 3/4" LARGE, 5/8"
national provisions apply. SMALL, 5/8" LARGE foil capsules.
2.2 Application 2.5 Base materials/Ancillary materials
The Hilti HUS4-MAX and KHC adhesive capsules together with Hilti HUS4-MAX and Hilti KHC are supplied in the form of
the Hilti mechanical anchors form the integrated Hilti HUS4- capsules. Product curing commences directly after the
MAX / Kwik-X Dual Action Anchor system which is used for components are mixed by drilling the capsule inside of the
fastenings of steel fixtures and machinery in cracked and borehole.
uncracked concrete. The adhesive capsules in the Dual Action The products reviewed in the EPD contain the following
Anchor system fill any voids around the screw anchor in the component values:
borehole which results in a better load transfer to the concrete
base material and thus in higher tensile loads. The HUS4-MAX Component A:
/ Kwik-X Dual Action Anchor system with the HUS4-MAX / KHC Methacrylate resin mixture: 90 to 100 % by weight
capsule is ICC-ES approved for cracked and uncracked Silica: 1 to 5 % by weight
concrete and all seismic design categories A-F. The adhesive Other: none
capsules are components of the Hilti SAFEset concept. It
significantly improves the robustness of fastening and Component B:
dramatically reduces the possibilities of error during installation. Water: 70 to 80 % by weight
As part of SAFEset the HUS4-MAX / Kwik-X Dual Action Dibenzoyl peroxide: 10 to 20 % by weight
Anchor system – comprising adhesive capsule and screw Other: <5 % by weight
anchor - can be installed with approved Hilti Hollow Drill bits
and vacuum cleaners that drill and clean the hole in one step This product
for virtually dust-free installation. Alternatively, it can be installed article contains substances listed in the candidate list (date:
in an uncleaned borehole if the drilling depth including a 20.01.2023) exceeding 0.1 percentage by mass: no.
specified overdrilling as described in the Instructions for Use is
adhered to. The preconfigured HUS4-MAX / KHC capsule This product
assures that there is the right amount of adhesive used for the The contains other Carcinogenic, Mutagenic, Reprotoxic (CMR)
fastening point (no under- or over-fill), thus reducing under- substances in categories 1A or 1B which are not on the
filling-related risks and eliminating adhesive wastage. candidate list, exceeding 0.1 percentage by mass: no.
2.3 Technical Data
Biocide
Constructional data products were added to this construction product or it has been
treated with biocide products (this then concerns a treated
product as defined by the Regulation (EU) No. 528/2012 on
biocidal products: no.
2 Environmental-Product Declaration - Hilti AG - HUS4-MAX and KHC
2.6 Manufacture 2.10 Condition of use
All raw materials are sourced in Europe or Asia. The transport During the installation the temperature of the concrete base
is exclusively by truck for the European raw materials, and by material must be between -28° C (-18° F) and +40° C (+104°
truck and by ship for the others. Chemical mortars are usually F). The temperature of the HUS4-MAX / KHC adhesive capsule
two-component systems consisting of a binder and a hardener. should be between +5° C (+41° F) to +25°C (+77° F) during
One of the base components of the binder is the reactive resin storage and +5° C (+41° F) to +40° C (+104° F) during
which in the case of HUS4-MAx and KHC is produced in installation. Hilti literature and official approvals must always be
Kaufering. considered. The two components of HUS4-MAX / KHC are only
The resin production process is a chemical reaction of the for use in combination with the defined volume ratio and under
corresponding educts to a basic resin with subsequent mixing the conditions mentioned above to build up a crosslinked
of the basic resin with different reactive diluents to a reactive duromer.
resin. This process is controlled and monitored by process
control technology. 2.11 Environment and health during use
The production of chemical mortars consists of a mixing Refer to the Safety Data Sheet (SDS) for detailed information
process and a filling process of the respective single on handling, storage as well as first aid, firefighting and
components (binder and hardener) and their subsequent union accidental release measures and disposal considerations.
to a two-component system (packaging). Here as well process Following the given instructions help to minimize the risk to
control technology is used to weigh and mix solid and liquid health and environment.
compounds according to the specification. In the next step both
2.12 Reference service life
well-mixed components run through an
automized filling line in which each of the processed masses is Hilti HUS4-MAX and KHC are exposed to a wide variety of
filled into a tubular foil bag. Finally, the single components are environmental factors during the use phase. The anticipated
combined in one packaging unit. The two-pack foil bags are Reference Service Life depends on the specific installation
packed into cardboard boxes and then finally shipped. situation and the product exposure scenario. The main factors
influencing the period of use involve weathering as well as
The manufacturing plant of HUS4-MAX and KHC, Hilti GmbH mechanical loads and chemical exposure.
Industriegesellschaft für Befestigungstechnik, Hiltistr. 6, 86916 Description of the influences on the ageing of the product when
Kaufering, Germany, is certified according to ISO 9001. The applied in accordance with the rules of technology.
guideline defines international standards for quality and
process management.
2.13 Extraordinary effects
2.7 Environment and health during manufacturing Fire
Even without any special fire safety features HUS4-MAX and
The manufacturing plant of HUS4-MAX and KHC,Hilti GmbH
KHC comply with at least the requirements of the DIN EN
Industriegesellschaft für Befestigungstechnik, Hiltistr. 6, 86916
13501-1 standard for fire classes E and Efl. As crosslinked
Kaufering, Germany, is certified according to ISO 14001 which
methacrylate resins do not melt or drip, the resins do not
defines international standards for sustainable environmental
contribute towards spreading fire. Apart from the common
management.
combustion that produces carbon monoxide and carbon
dioxide, fire gases can contain traces of methyl methacrylate,
The production site is also certified in accordance with ISO
esters, alcohol, and hydrocarbons. Due to the quantities used,
50001 Energy Management Systems.
they only have a subordinate influence on the fire
2.8 Product processing/Installation characteristics of a building structure in which they have been
The product is delivered with Instructions for Use explaining the installed.
basic steps for installation: Fire protection
1) For safe handling the precautionary measures described in
Name Value
the Safety Data Sheet (SDS) (e.g. hand and eye protection)
Building material class E/Efl
must be adhered to
2) Select the correct capsule size based on the diameter of the Burning droplets No performance assessed
screw anchor and the embedment depth Smoke gas development No performance assessed
2) Insert the capsule into the borehole
3) Mixing the two components of the capsule by driving the
Water
screw anchor with a suitable impact wrench into
The cured products are chemically inert and insoluble in water.
the borehole
HUS4-MAX and KHC are certified for use as an anchoring
adhesive in concrete for water treatment applications according
After mixing the components of the HUS4-MAX / KHC capsule
to National Sanitation Foundation (US) NSF.
in the borehole partial load (not exceeding the load capacity of
the screw anchor) can be applied immediately. The full load up
Mechanical destruction
to the capacity of the HUS4-MAX / Kwik-X Dual Action Anchor
It is recommended to use dust protection during the demolition
system can be applied after the curing time of the HUS4-MAX /
of the cured chemical anchor.
KHC adhesive mentioned in the Instructions for Use.
2.14 Re-use phase
2.9 Packaging
The product cannot be reused. After usage the product can be
The Hilti HUS4-MAX / KHC adhesive foil capsules are installed
removed by demolition.
and remain in the borehole. Thus, no waste is remaining after
use on the construction site. The sales packaging consisting of 2.15 Disposal
a cardboard box designed according to the product size and
Uncured Hilti HUS4-MAX and KHC can be disposed according
packaging quantity and can be recycled. Packaging
to the European waste code 08 04 09* or 20 01 27*. The built-in
contaminated by the product must be disposed in a safe
cured anchor can be disposed as construction waste for which
manner in accordance with local / national regulations.
the European waste code 17 01 01 applies.
3 Environmental-Product Declaration - Hilti AG - HUS4-MAX and KHC
anchor.hse@hilti.com and on the Hilti website:
2.16 Further information www.hilti.group
Further information is available on request under
3. LCA: Calculation rules
3.1 Declared Unit
The notified product is an injection mortar of HILTI AG with the
designation HUS4-MAX 12 as a representative product from
the HUS4-MAX and KHC portfolio, as only the packaging
proportions change per 1 kilogram of injection mortar. The
declared unit refers to 1 kg of reaction resin product in the
mixing ratio of the two components required for processing. The
packaging, related to 1 kg injection mortar, is additionally
included in the calculation with 0.355 kg. The following table
shows the data of the declared unit.
Declared unit
Name Value Unit
Declared unit 1 kg
Conversion factor to 1 kg 1
3.2 System boundary Illustration 1: Information module A1 to A3 of
Type of EPD: product (part 1)
cradle to gate with options.The following information modules
are defined as system boundaries in this study:
Production stage (A1- A3):
• A1, raw material extraction,
• A2, transport to manufacturer,
• A3, manufacture. Illustration 2:
Information module A1 to A3 of product (part 2)
End of life
(C1- C4):
• C1, dismantling/demolition,
• C2, transportation,
• C3, waste treatment,
• C4, elimination. Illustration 3:
Information module A1 to A3 of packaging
Reuse, recovery
and recycling potential (D)
In the information modules C1 to C4, the deconstruction or
demolition from the building, the transport to waste disposal,
In order to precisely record the indicators and environmental the waste treatment and disposal of the product are recorded.
impacts of the declared unit, a total of 8 information modules Furthermore, reuse, recovery and recycling potentials are
are considered. The information modules A1 to A3 describe the shown in information module D.
provision of materials, the transport to the production site and
the production processes of the product itself.
The primary products are sourced from the European Union 3.3 Estimates and assumptions
and Asia .Transport is by truck and ship. The following flow The electricity mixes and other background data are calculated
charts illustrate the underlying production process. country-specifically for the production processes.
No assumptions or restrictions were made for the recipe
contents or processes.
3.4 Cut-off criteria
All energy and mass inputs were taken into account.The cut-off
criterion according to EN 15804+A2 is not applied.
3.5 Background data
4 Environmental-Product Declaration - Hilti AG - HUS4-MAX and KHC
The database of the background data of the LCA for Experts lifespan: Germany
and ecoinvent 3.8 databases, to which this study also refers, is
documented under the following link. (Sphera)
3.9 Allocation
3.6 Data quality Allocation of co-products takes place in the information
For the preparation of the life cycle assessment, the annual modules A1-A3. The production waste of the injection-moulded
average consumption of HILTI AG from the Kaufering plant in components is thermally recovered. The electrical and thermal
Germany was collected. The background data from the LCA for energy credits resulting therefrom are completely charged in
Experts database are from the year 2023 and are therefore modules A1-A3. No further allocations are made.
highly relevant. The masses of the various components of the
3.10 Comparability
reaction resin mixture are taken from the recipe data. The data
quality is rated as sufficient. Basically, a comparison or an evaluation of EPD data is only
possible if all the data sets to be compared were created
3.7 Period under review according to EN 15804 and the building context, respectively
The input and output flows used in this calculation are annual the product-specific characteristics of performance, are taken
average consumptions from 2018 to 2021. into account. The database with background data from the LCA
for Experts and ecoinvent 3.8 databases, to which this study
3.8 Geographic Representativeness also refers
Land or region, in which the declared product system is
manufactured, used or handled at the end of the product´s
4. LCA: Scenarios and additional technical information
The product is demolished using an electric chisel. The
Characteristic product properties biogenic carbon electrical energy consumption for the tool is assumed to be
No renewable raw materials are used in the product. Therefore, 0.05 MJ for the declared unit. The electricity consumption is
the biogenic carbon is shown as zero. The following raw calculated with a European electricity mix. The construction
materials contain biogenic carbon in the packaging. waste is transported by truck 50 km to the waste treatment
Information on describing the biogenic Carbon Content at plant. The construction waste is shredded in the waste
factury gate treatment plant and then dumped.
Name Value Unit Name Value Unit
Packaging Cardboard Box 0,081 kg C Collected as mixed construction waste 1 kg
Packaging Paper 0,027 kg C Crushing in the shredder 1 kg
Landfilling 1 kg
Reuse, recovery and/or recycling potentials (D), relevant
Information on packaging scenario information
Name Value Unit In this calculation there are no reuse, recovery and recycling
potentials. Therefore, the information module D is declared and
Composite foil PP/PA/PE 0,1017 kg
shown as zero.
Paper 0,0639 kg
Name Value Unit
Cardboard box 0,1902 kg
Reuse, recovery and recycling potentials 0 kg
End of life (C1-C4)
5 Environmental-Product Declaration - Hilti AG - HUS4-MAX and KHC
5. LCA: Results
DESCRIPTION OF THE SYSTEM BOUNDARY (X = INCLUDED IN LCA; ND = MODULE OR INDICATOR NOT DECLARED; MNR =
MODULE NOT RELEVANT)
Benefits and
Construction loads beyond
Product stage Use stage End of life stage
process stage the system
boundaries
la ire ta m w a Ry lp p u s tro p s n a rT g n iru tc a fu n a M e h t m o rf tro p s n a rTe tis e h t o t e ta g y lb m e s s A e s U e c n a n e tn ia M ria p e R tn e m e c a lp e R tn e m h s ib ru fe R y g re n e la n o ita re p Oe s u re ta w la n o ita re p Oe s u n o itc u rts n o c -e Dn o itilo m e d tro p s n a rT g n is s e c o rp e ts a W la s o p s iD -e s u e R-y re v o c e R-g n ilc y c e Rla itn e to p
A1 A2 A3 A4 A5 B1 B2 B3 B4 B5 B6 B7 C1 C2 C3 C4 D
X X X MND MND MND MND MNR MNR MNR MND MND X X X X X
RESULTS OF THE LCA - ENVIRONMENTAL IMPACT according to EN 15804+A2: 1 kg HILTI HUS4-MAX 12
Parameter Unit A1-A3 C1 C2 C3 C4 D
Global Warming Potential total (GWP-total) kg CO 2 eq 6.21E+00 5.12E-03 3.76E-03 2.68E-03 1.49E-02 0
Global Warming Potential fossil fuels (GWP-fossil) kg CO 2 eq 6.21E+00 5.12E-03 3.74E-03 2.67E-03 1.49E-02 0
Global Warming Potential biogenic (GWP-biogenic) kg CO 2 eq 0 0 0 0 0 0
Global Warming Potential luluc (GWP-luluc) kg CO 2 eq 3.71E-03 1.08E-06 2.07E-05 1.23E-05 2.75E-05 0
Depletion potential of the stratospheric ozone layer (ODP) kg CFC11 eq 1.59E-07 7.5E-14 2.22E-16 3.97E-15 3.51E-14 0
Acidification potential of land and water (AP) mol H+ eq 2.86E-02 1.12E-05 1.17E-05 1.38E-05 1.06E-04 0
Eutrophication potential aquatic freshwater (EP-freshwater) kg P eq 8.81E-04 1.49E-08 1.11E-08 7.66E-09 2.53E-08 0
Eutrophication potential aquatic marine (EP-marine) kg N eq 5.92E-03 2.52E-06 5.37E-06 6.29E-06 2.71E-05 0
Eutrophication potential terrestrial (EP-terrestrial) mol N eq 5.42E-02 2.65E-05 6.01E-05 6.95E-05 2.97E-04 0
Formation potential of tropospheric ozone photochemical oxidants kg NMVOC
1.75E-02 6.82E-06 1.05E-05 1.71E-05 8.22E-05 0
(POCP) eq
Abiotic depletion potential for non fossil resources (ADPE) kg Sb eq 8.85E-05 1.4E-09 3.1E-10 2.96E-09 1.53E-09 0
Abiotic depletion potential for fossil resources (ADPF) MJ 1.18E+02 9.29E-02 4.96E-02 5.21E-02 1.95E-01 0
m3 world eq
Water use (WDP) 2.69E+00 1.17E-03 3.33E-05 5.15E-04 1.64E-03 0
deprived
RESULTS OF THE LCA - INDICATORS TO DESCRIBE RESOURCE USE according to EN 15804+A2: 1 kg HILTI HUS4-MAX 12
Parameter Unit A1-A3 C1 C2 C3 C4 D
Renewable primary energy as energy carrier (PERE) MJ 1.19E+01 5.16E-02 2.82E-03 4.19E-03 2.93E-02 0
Renewable primary energy resources as material utilization
MJ 3.81E+00 0 0 0 0 0
(PERM)
Total use of renewable primary energy resources (PERT) MJ 1.57E+01 5.16E-02 2.82E-03 4.19E-03 2.93E-02 0
Non renewable primary energy as energy carrier (PENRE) MJ 1.06E+02 9.3E-02 4.97E-02 5.23E-02 1.96E-01 0
Non renewable primary energy as material utilization (PENRM) MJ 1.24E+01 0 0 0 0 0
Total use of non renewable primary energy resources (PENRT) MJ 1.18E+02 9.3E-02 4.97E-02 5.23E-02 1.96E-01 0
Use of secondary material (SM) kg 2.8E-01 0 0 0 0 0
Use of renewable secondary fuels (RSF) MJ 0 0 0 0 0 0
Use of non renewable secondary fuels (NRSF) MJ 0 0 0 0 0 0
Use of net fresh water (FW) m3 7.03E-02 4.92E-05 3.19E-06 1.46E-05 4.97E-05 0
RESULTS OF THE LCA – WASTE CATEGORIES AND OUTPUT FLOWS according to EN 15804+A2:
1 kg HILTI HUS4-MAX 12
Parameter Unit A1-A3 C1 C2 C3 C4 D
Hazardous waste disposed (HWD) kg 8.28E-08 8.04E-12 2.38E-13 6.53E-13 1.01E-11 0
Non hazardous waste disposed (NHWD) kg 4.43E-02 7E-05 7.13E-06 1.39E-05 1E+00 0
Radioactive waste disposed (RWD) kg 1.09E-03 1.49E-05 6.13E-08 6.88E-07 2.18E-06 0
Components for re-use (CRU) kg 0 0 0 0 0 0
Materials for recycling (MFR) kg 0 0 0 0 0 0
Materials for energy recovery (MER) kg 0 0 0 0 0 0
Exported electrical energy (EEE) MJ 0 0 0 0 0 0
Exported thermal energy (EET) MJ 0 0 0 0 0 0
RESULTS OF THE LCA – additional impact categories according to EN 15804+A2-optional:
1 kg HILTI HUS4-MAX 12
Parameter Unit A1-A3 C1 C2 C3 C4 D
Disease
Incidence of disease due to PM emissions (PM) ND ND ND ND ND ND
incidence
Human exposure efficiency relative to U235 (IR) kBq U235 eq ND ND ND ND ND ND
Comparative toxic unit for ecosystems (ETP-fw) CTUe ND ND ND ND ND ND
Comparative toxic unit for humans (carcinogenic) (HTP-c) CTUh ND ND ND ND ND ND
Comparative toxic unit for humans (noncarcinogenic) (HTP-nc) CTUh ND ND ND ND ND ND
6 Environmental-Product Declaration - Hilti AG - HUS4-MAX and KHC
Soil quality index (SQP) SQP ND ND ND ND ND ND
The secondary material (SM) used leads from paper production.
Disclaimer 2 – for the indicators 'abiotic depletion potential for non-fossil resources', 'abiotic depletion potential for fossil resources',
'water (user) deprivation potential, deprivation-weighted water consumption', 'potential comparative toxic unit for ecosystems', 'potential
comparative toxic unit for humans – cancerogenic', 'Potential comparative toxic unit for humans - not cancerogenic', 'potential soil
quality index'.
The results of this environmental impact indicator shall be used with care as the
uncertainties on these results are high or as there is limited experienced with the indicator.
6. LCA: Interpretation
Dominance analysis All modules Illustration:Dominance analysis A1
The dominance analysis shows that the main causes of Dominance analysis A1, reaction resin mixture
environmental impacts and indicators are to be found in
information module A1. This can be seen in the total global Within the reaction resin mixture itself, the material supply of
warming potential for material supply with approx. 93%, related the Butanedioldimethacrylate (BDDMA) generates approx. 75%
to all information modules. For the total non-renewable primary of the total global warming potential and approx. 72% of the
energy, the value is approx. 96%. Modules C1 to C4 are total non-renewable primary energy. The UMA 121 has a share
negligible in this analysis, accounting for approx. 1% of the total of approx. 15% of the total greenhouse gas emissions and
global warming potential. approx. 18% of the total non-renewable primary energy.
Illustration:Dominance analysis A1- A3
Dominance analysis A1
Illustration:Dominance analysis A1, reaction resin mixture
If we look at the material supply of the reaction resin mixture
and the packaging in detail, it becomes clear which raw As this is a representative product for a portfolio, the
materials contribute decisively to the respective environmental environmental impact of the packaging may change. The
impacts and indicators. environmental impact of the reaction resin on 1kg does not
change.
The reaction resin mixture itself accounts for 92% of the total
global warming potential in information module A1. The
cardboard box accounts for approx. 3% and the composite foil
for approx. 3%.
7. Requisite evidence
Hilti HUS4-MAX complies with the requirements of · CDPH/EHLB Standard Method V 1.2 (2017) in
· DIBt (2010) in combination with the NIK values accordance with Eurofins test report, No. 392-2021-
from AgBB (2021) for applications in interior areas, 00413604_CA_EN, Eurofins test report, No. 392-2021-
· emission class A+ outlined in the French VOC 00413604_E_EN and Eurofins test report, No. 392-2021-
Directives (2019) in accordance with the Eurofins attestation, 00413602_H_EN respectively.
7 Environmental-Product Declaration - Hilti AG - HUS4-MAX and KHC
Hilti KHC complies with the requirements of Name Value Unit
· CDPH/EHLB Standard Method V 1.2 (2017) in TVOC (C6 - C16) <1000 μg/m3
accordance with Eurofins test report, No. 392-2021-
Sum SVOC (C16 - C22) <100 μg/m3
00413602_H_EN.
R (dimensionless) <1 -
AgBB overview of results (28 days [µg/m³])
VOC without NIK <100 μg/m3
Carcinogenic Substances <1 μg/m3
8. References
EN ISO 604 ecoinvent 3.8
EN ISO 604: 2003-12, Kunststoffe - Bestimmung von Backgroun data: ecoinvent 3.8
Druckeigenschaften Zürich:
ecoinvent
EN 13501-1 http://www.ecoinvent.org
EN 13501-1: 2019-05, Klassifizierung von Bauprodukten und (10.05.2023)
Bauarten zu ihrem Brandverhalten - Teil 1: Klassifizierung mit
den Ergebnissen aus den Prüfungen zum Brandverhalten von ETA 18/1160
Bauprodukten European Technical Approval Hilti HUS4
Eurofins test report, No. 392-2021-00413604_CA_EN
EN 15804 VOC test report for verification of compliance with
EN 15804+A2:2019+AC:2021, Sustainability of construction DIBt(2010)/AgBB(2021)
works — Environmental Product Declarations — Core rules for
the product category of construction products Eurofins test report, No. 392-2021-00413604_E_EN
VOC test report for verification of compliance with the French
ISO 14001 directive from 2010
ISO 14001: 2015-09, Umweltmanagementsysteme -
Anforderungen mit Anleitung zur Anwendung Eurofins test report, No. 392-2021-00413602_H_EN
VOC test report for verification of compliance with
ISO 14025 CDPH/EHLB/Standard Method V1.2 from 2017
DIN EN /ISO 14025:2011-10/, Environmental labels and
declarations — Type III environmental declarations — European Waste code
Principles and procedures in accordance with the European Waste Catalogue (EWC)
(EWC 2014/955/EU) Commission Decision amending Decision
ISO 50001 2000/532/EC on the list of waste pursuant to Directive
ISO 50001: 2018-08, Energiemanagementsysteme - 2008/98/EC of the European Parliament and of the Council
Anforderungen mit Anleitung zur Anwendung
French VOC Directives
ISO 9001 Décret no 2011321 du 23 mars 2011 relatif à l'étiquetage des
ISO 9001: 2015-11, Qualitätsmanagementsysteme - produits de construction ou de revêtement de mur ou de sol et
Anforderungen des peintures et vernis sur leurs émissions de polluants volatils
Arrêté du 19 avril 2011 relatif à l'étiquetage des produits de
AgBB (2021) construction ou de revêtement de mur ou de sol et des
Vorgehensweise bei der gesundheitlichen Bewertung der peintures et vernis sur leurs émissions de polluants volatils
Emissionen von flüchtigen organischen Verbindungen (VVOC,
VOC und SVOC) aus Bauprodukten (2021) IBU 2021
General Instructions for the EPD programme of Institut Bauen
Candidate List of substances of very high concern for und Umwelt e.V. Version 2.0,
Authorisation Berlin: Institut Bauen und Umwelt e.V.,2021
European Cheminals Agency (ECHA), in accordance with www.ibu-epd.de
Article 50(10) of the REACH regulation
ICC ESR-5065
CDPH/EHLB/Standard Method V1.2 International code council (ICC), Evaluation report ESR-5065
California CDPH Standard Method is a US standard for HILTI KWIK-X (December 2022)
evaluating and restricting VOC emissions to indoor air.
Developed in California as "Section 01350" Specification, Product category rules for construction products – Part B
several systems in the US refer to CDPH Standard Method Reaction resin products, 04.2023
Calculation rules: PCR - Part A Regulation (EU) No. 305/2011 (CPR)
Institut Bauen und Umwelt e.V. (IBU), 2022. Product Category Regulation (EU) No 305/2011 of the European Parliament and
Rules for Building-Related Products and Services. Part A: of the Council of 9 March 2011 laying down harmonised
Calculation rules for the life cycle assessment and conditions for the marketing of construction products and
requirements on the project report. Version 1.3 (08.2022) repealing Council Directive 89/106/EEC Text with EEA
relevance
DIBt (2010)
Grundsätze zur gesundheitlichen Bewertung von Bauprodukten Regulation (EU) No. 528/2012
in Innenräumen (Oktober 2010) REGULATION (EU) No 528/2012 OF THE EUROPEAN
PARLIAMENT AND OF THE COUNCIL of 22 May
8 Environmental-Product Declaration - Hilti AG - HUS4-MAX and KHC
2012concerning the making available on the market and use of LCA for Experts, Leinfelden-Echterdingen; Sphera Solution
biocidal products Text with EEA relevance GmbH,
https://gabi.sphera.com/databases/gabi-data-search/
Sphera (10.05.2023)
9 Environmental-Product Declaration - Hilti AG - HUS4-MAX and KHC
Publisher
Institut Bauen und Umwelt e.V. +49 (0)30 3087748- 0
Hegelplatz 1 info@ibu-epd.com
10117 Berlin www.ibu-epd.com
Germany
Programme holder
Institut Bauen und Umwelt e.V. +49 (0)30 3087748- 0
Hegelplatz 1 info@ibu-epd.com
10117 Berlin www.ibu-epd.com
Germany
Author of the Life Cycle Assessment
FIT-Umwelttechnik GmbH 05362 72 69 474
Westerstr. 13 bertram@fit-umwelttechnik.de
38442 Wolfsburg www.fit-umwelttechnik.com
Germany
Owner of the Declaration
Hilti Aktiengesellschaft +423 234 2111
Feldkircher Strasse 100 HAGHSE@hilti.com
9494 Schaan www.hilti.com
Liechtenstein
10 Environmental-Product Declaration - Hilti AG - HUS4-MAX and KHC
