ENVIRONMENTAL PRODUCT DECLARATION
as per ISO 14025 and EN 15804+A2
Owner of the Declaration
Programme holder Institut Bauen und Umwelt e.V. (IBU)
Publisher Institut Bauen und Umwelt e.V. (IBU)
Declaration number EPD­HIL­20220124­IBA1­EN
Issue date 21.06.2022
Valid to 20.06.2027
Hilti HVU2
HILTI AG
www.ibu-epd.com | https://epd-online.com
Umwelt Produktdeklaration Name des Herstellers – Name des Produkts
1. General Information
HILTI AG HVU2
Programme holder Owner of the declaration
IBU – Institut Bauen und Umwelt e.V. Hilti AG
Hegelplatz 1 Feldkircher Str. 100
10117 Berlin FL­9494 Schaan
Germany Liechtenstein
Declaration number Declared product / declared unit
EPD­HIL­20220124­IBA1­EN The declared product is HILTI’s HVU2 adhesive
capsule. The declared unit is one kilogram of reaction
resin product. The packaging is also included in the
calculation. The declared unit is stated in [kg]
This declaration is based on the product Scope:
category rules: This document refers to the adhesive capsule
Reaction resin products, 11.2017 HVU2 with its packaging. For the compilation of the
(PCR checked and approved by the SVR) life cycle assessment, specific data were collected
from the factory in Kaufering, Germany, of the HILTI
AG. Data from the year 2019 are used, which
Issue date
correspond to the annual average.
21.06.2022
The owner of the declaration shall be liable for the
Valid to
underlying information and evidence; the IBU shall not
20.06.2027
be liable with respect to manufacturer information, life
cycle assessment data and evidences.
The EPD was created according to the specifications
of EN 15804+A2. In the following, the standard will be
simplified as EN 15804.
The owner of the declaration shall be liable for the
underlying information and evidence; the IBU shall not
be liable with respect to manufacturer information, life
cycle assessment data and evidences.
The EPD was created according to the specifications
of EN 15804+A2. In the following, the standard will be
simplified as EN 15804.
Verification
The standard EN 15804 serves as the core PCR
Independent verification of the declaration and data
according to ISO 14025:2011
Dipl. Ing. Hans Peters internally x externally
(chairman of Institut Bauen und Umwelt e.V.)
Dr. Alexander Röder Matthias Klingler
(Managing Director Institut Bauen und Umwelt e.V.)) (Independent verifier)
2. Product
2.1 Product description/Product definition bond strengths within short curing time) and particular
long­term stability.
The declared product of HVU2 is a two­component Composite foils are used for the HVU2 capsule. This
system. kind of packaging serves the following purposes: waste
The resin component comprises a resin based on volume reduction, easy storage and transport, less
methacrylates as well as mineral fillers. The curing packaging material.
agent component comprises of peroxide hardener. Through legislation and increased public awareness
Mixing the two components in the borehole initiates the users have increasingly become discerned towards the
curing (hardening) reaction of both binder systems. use of styrene and other highly volatile components
During the curing phase a very strong bond is formed. with their resulting unpleasant odour and low flash
The system formed during curing results in a cross­ point (flammability).
linked duromer with desired design properties (high The reaction resins used in all Hilti hybrid adhesives
contain no styrene, are practically odourless and have
2 Environmental Product Declaration Hilti AG – HVU2
a considerably higher flash point, i.e. higher than 100 2.4 Delivery status
°C in comparison to 34 °C for styrene­based products. The product Hilti HVU2 is available in M8x80, M10x90,
HVU2 is the ultimate performance foil adhesive M10x135, M12x110, M12x165, M16x125, M16x190,
capsule for heavy­duty anchoring in concrete. M20x125, M20x170, M24x210, M27x240, M30x270,
For the placing of the product on the market in the 3/8" x 3 1/2", 1/2" x 4 1/4", 5/8" x 5", 3/4" x 6 5/8", 7/8"
European Union European Free Trade Association x 6 5/8", 1" x 8 1/4", 1 1/4" x 11" foil­capsules.
EU/EFTA) (with the exception of Switzerland) the
Regulation (EU) No. 305/2011 (CPR) applies. The 2.5 Base materials/Ancillary materials
product needs a declaration of performance taking into Hilti HVU2 is supplied in the form of a capsule.
consideration the following European Technical Product curing commences directly after the
Approval ETA 16/0515 and the CE­marking. For the components are mixed by drilling the capsule inside of
application and use the respective national provisions the borehole.
apply.
The product reviewed in this EPD contains the
2.2 Application following component volumes:
Hilti HVU2 serves for safely securing of threaded rods
in cracked and uncracked concrete C20/25 to C50/60. Components of the capsule:
HVU2 is ETA and ICC approved for seismic C1 and C2 Methacrylate resin mixture: 10 to 20% by weight
category for anchoring and C1 category for rebar. Mineral fillers: 80 to 90% by weight
Dibenzoyl peroxide: 0,5 to <1,5% by weight
The HVU2 is an extremely universal product for Other: <5% by weight
various anchoring applications. Its range technical data
is wide, extending from cracked concrete, diamond This product article contains substances listed in the
coring (both cracked and uncracked) and workability candidate list (date: 25.04.2022) exceeding 0.1
with Hilti Hollow Drill Bit (SafeSet) in light steel percentage by mass: yes; Dicyclohexyl phthalate
construction to extremely heavy­duty fastenings. (DCHP) (EC 201­545­9, CAS 84­61­7), below 1,5 %
by weight.
2.3 Technical Data This product contains other CMR substances in
categories 1A or 1B which are not on the candidate
list, exceeding 0.1 percentage by mass: yes,
Constructional data dicyclohexyl phthalate (CAS 84­61­7), classified as
Name Value Unit Repr. 1B, H360D, below 1,5 % by weight.
Density EN ISO 1183­1 2950 kg/m3
Compressive strength Biocide products were added to this construction
77 N/mm^2
(Tcure=120h) EN ISO 604 product or it has been treated with biocide products
Elastic modulus (pressure) EN (this then concerns a treated product as defined by the
3100 N/mm^2
ISO 604 (EU) Ordinance on Biocide Products No. 528/2012):
Tensile shear strength acc. to DIN not no.
N/mm2
EN 14293 relevant
Tensile bond strength acc. to DIN not
N/mm2
EN 14293 relevant 2.6 Manufacture
Most raw materials are sourced in Europe. The
transport is exclusively by truck for the European raw
Hilti HVU2 displays the following characteristics: materials, and by truck and by ship for the others.
Chemical mortars are usually two­component systems
Performance data of the product in accordance with consisting of a binder and a hardener. One of the base
the declaration of performance with respect to its components of the binder is the reactive resin which in
essential characteristics according to ETA 16/0515. the case of HVU2 is produced in Kaufering. The resin
Shelf life of 12 months: production process is a chemical reaction of the
Substrate temperature during installation ­10 to +40 °C corresponding educts to a basic resin with subsequent
(internal method). mixing of the basic resin with different reactive diluents
to a reactive resin. This process is controlled and
Working time: monitored by process control technology.
­10 to ­5 °C 5 h The production of chemical mortars consists of a
> ­5 to 0 °C 3 h mixing process and a filling process of the respective
> 0 to +5 °C 40 min single components (binder and hardener) and their
> 5 to +10 °C 20 min subsequent union to a two­component system
> 10 to +20 °C 10 min (packaging). Here as well process control technology
> 20 to +40 °C 5 min is used to weigh and mix solid and liquid compounds
according to the specification. In the next step both
Curing time: well­mixed components run through an automized
­10 to ­5 °C 5 h filling line in which each of the processed masses is
> ­5 to 0 °C 3 h filled into a tubular foil bag. Finally the single
> 0 to +5 °C 40 min components are combined in one packaging unit. The
> 5 to +10 °C 20 min two­pack foil bags are packed into cardboard boxes
> 10 to +20 °C 10 min and then finally shipped. The manufacturing plant of
> 20 to +40 °C 5 min HVU2, Hilti GmbH Industriegesellschaft für
Befestigungstechnik, Hiltistr. 6, 86916 Kaufering,
Germany, is certified according to ISO 9001. The
3 Environmental Product Declaration Hilti AG – HVU2
guideline defines international standards for quality
and process management. 2.10 Condition of use
The following flowcharts illustrate the underlying During the installation the temperature of the base
production process. material must be between ­10°C and +40°C . The
temperature of the product should be between ­20 and
+25 °C during storage and ­10 and +40°C during
usage. Hilti literature and official approvals must
always be considered. The two components of HVU2
are only for use in combination with the defined volume
ratio and under these conditions mentioned above to
build up a cross­linked filled duromer.
2.11 Environment and health during use
Refer to the Safety Data Sheet (SDS) for detailed
information on handling, storage as well as first aid,
Illustration: Production process of the reaction
firefighting and accidental release measures and
resin mixture
disposal considerations. Following the given
instructions helps to minimize the risk for health and
environment.
2.12 Reference service life
Hilti HVU2 is exposed to a wide variety of
environmental factors during the use phase. The
anticipated Reference Service Life depends on the
specific installation situation and the product exposure
Illustration: Production process of the packaging
scenario. The main factors influencing the period of
use involve weathering as well as mechanical loads
2.7 Environment and health during
and chemical exposure.
manufacturing
The manufacturing plant of HVU2,Hilti GmbH
Industriegesellschaft für Befestigungstechnik, Hiltistr.
2.13 Extraordinary effects
6, 86916 Kaufering, Germany, is certified according to
ISO 14001 which defines international standards for
Fire
sustainable environmental management. The
Fire resistance of the anchor system Hilti HVU2 under
production site is also certified in accordance with DIN
fire exposure acc. DIN EN 1363­1 has been tested by
EN ISO 50001 Energy Management Systems.
Ing. Thiele, Pirmasens, report 21735.
2.8 Product processing/Installation
Water
The product is delivered with Instructions for Use
The cured product is chemically inert and insoluble in
explaining the basic steps for installation:
water. HVU2 is certified for use as an anchoring
adhesive in concrete for water treatment applications
1) For safe handling the precautionary measures
according to National Sanitation Foundation (US)
described in the SDS (e.g. hand and eye protection)
/NSF/.
must be adhered to
2) Insert the capsule into the borehole.
Mechanical destruction
3) Mix it with a driller
It is recommended to use dust protection during
demolition of the cured chemical anchor.
After the curing time, described as well in Instructions
for Use, the mortar is ready to take up loads.
2.14 Re-use phase
The product cannot be re­used. After usage the
2.9 Packaging
product can be removed by demolition.
Hilti HVU2 is supplied in the form capsule packaging
which is not removed before use and thus leads to no
2.15 Disposal
waste remaining after use on the construction site.
Uncured Hilti HVU2 can be disposed of according to
The outer packaging consisting of plastic foil and
the European waste code 08 04 09* or 20 01 27*. The
cardboard boxes designed according to the product
built­in cured anchor can be disposed as construction
size can be recycled. Packaging contaminated by the
waste for which the European waste code 17 01 01
product must be disposed in a safe manner in
applies.
accordance with local/national regulations.
For this EPD, the declared packaging is a weighted
2.16 Further information
meanvalue of all available packaging sizes. This
Further information is available on request under
results in a 224 g packaging composed of 30 g of
anchor.hse@hilti.com and on the Hilti website:
plastic, 194 g of paper and cardboard.
www.hilti.group
3. LCA: Calculation rules
3.1 Declared Unit the two components. The packaging of 0,224 kg/kg of
The declared product is a HILTI adhesive capsule product is also included in the calculation. The
HVU2. The declared unit refers to one kilogram of following table shows the data of the declared unit.
reaction resin product in the required mixing ratio of
4 Environmental Product Declaration Hilti AG – HVU2
Declared unit were used to reconstructed these material's
Name Value Unit impact
Declared unit 1 kg
 Some raw material's packaging composition
and transportation distances were estimated
 The energy consumption for production of the
3.2 System boundary current product (HVU2) was assimilated to
The type of the EPD is cradle to grave. The following the energy consumption measured on the
information modules are defined as system boundaries production line of another Hilti product, which
in this study: has a very similar manufacturing process
 Estimations were made to calculate the
A1 – Raw material supply:
energy consumption during installation
Production and packaging of the raw materials to be
supplied to the manufacturer. All processes are  The transportation scenario to building site is
included from cradle to gate. based on french transportation companies
A2 – Transport (to manufacturing site): statistics.
Transportation of all the raw materials and their
packaging between their production site and the
manufacturing site, for all transport modes (sea, road).
3.4 Cut-off criteria
A3 – Manufacturing:
All information modules considered were included in
Production, supply and use of energy sources at the
the calculation in such detail that all requirements of
manufacturing sites (electricity, biomass and natural
/EN 15804/ are met. The consumption of additional
gas). Green electricity from wind turbines is
inputs such as lubricants, oils or solvents used for
considered for the whole manufacturing process.
manufacture is less than 5% by weight and therefore
Production and transport of production losses, final
falls below the cut­off criterion of the total calculation.
product packaging and other inputs.
End­of­life of production waste (hazardous, non­
3.5 Background data
hazardous and recyclable), production losses and raw
The source for background data for the LCA
material packaging, including waste and losses
calculations is the ecoinvent 3.8 database.
transportation, processing and disposal.
A4 – Transport (to construction site)
3.6 Data quality
Transportation of packaged products from the
For the compilation of the life cycle assessment,
manufacturing site to the construction site, including
specific data were collected from the factory Kaufering,
potential in­betweens (retailer, workshop, etc.).
in Germany, of the HILTI AG from the year 2019. The
A5 – Installation­Construction
background data from the ecoinvent 3.8 database
Electricity consumption for mixing.
used was updated in the year 2021 and thus of highly
End­of­life of non­hazardous construction losses
up­to­date. The mass of the different components of
(cured mortar and unsoiled packaging): including
the reactive resin mixture come from the information in
waste transportation, processing and disposal.
the recipe. The data quality is classified as appropriate.
C1 – Deconstruction/demolition
Diesel for building demolition.
3.7 Period under review
C2 – Transport (to waste processing)
Data from the year 2019 are used, which correspond
Transportation to waste processing facility.
to the annual average.
C4– Waste disposal
Treatment and disposal of plastic to sanitary landfill.
3.8 Allocation
The energy for manufacturing (A3) is supposed to be
For the environmental impact, the use of green
the same as for another HITLI product, which
electricity (stage A3) was calculated taking into
consumptions were measured on production line. No
account the residual electricity mix for the remaining
allocation was used for this stage.
electricity. The proportion of the electricity demand
covered by green electricity in the total electricity
3.9 Comparability
demand is 100%.
Basically, a comparison or an evaluation of EPD data
is only possible if all the data sets to be compared
3.3 Estimates and assumptions
were created according to EN 15804 and the building
In general, background data and elecricity mixes are
context, respectively the product­specific
chosen and calculated country­specifically for the
characteristics of performance, are taken into account.
production processes. In some cases, assumptions
were made because of a lack of primary or secondary
The used background database is given by ecoinvent
data, in particular for the following aspects:
3.8 database, to which this study refers.
 The synthesis way of raw materials which
were not available on the Ecoinvent database
4. LCA: Scenarios and additional technical information
Characteristic product properties packaging, all the biogenic carbon capture and release
Information on biogenic Carbon were cancelled to simplify the model.
The declared product contains 194 g of paper and The cancelled emission corresponds to 0,025 kg of
cardboard (outer packaging and user manual). Since biogenic carbon (0,0954 kg of CO2) for a cancelled
only this materials contain biogenic carbon, in addition capture of 0,047 kg of biogenic carbon (0,1783 kg of
to a neglectable part contained in the raw material CO2).
5 Environmental Product Declaration Hilti AG – HVU2
The following scenarios were considered for the LCA
calculations:
Transport to the building site (A4)
Name Value Unit
Transport distance 900 km
lorry 16­
32
Vehicle type ­
metric
ton
Effective load 21 t
Maximum capacity 24 t
Consumption when unloaded 0,25 L/km
Consumption at fill capacity 0,38 L/km
Empty return rate 14 %
Effective consumption 0,019 L/tkm
Installation into the building (A5)
Name Value Unit
Electricity consumption 0.264 kWh
Uncured mortar loss 0 kg
Cured mortar loss 0 kg
Material loss 0 kg
Hazardous waste (soiled
0 kg
packaging)
Non­hazardous waste (unsoiled
0,216 kg
packaging)
End of life (C1-C4)
Name Value Unit
Fuel for building demolition 0,0437 MJ
Distance to sanitary landfill 50 km
Landfilling 1.03 kg
6 Environmental Product Declaration Hilti AG – HVU2
5. LCA: Results
DESCRIPTION OF THE SYSTEM BOUNDARY (X = INCLUDED IN LCA; ND = MODULE OR INDICATOR NOT
DECLARED; MNR = MODULE NOT RELEVANT)
BENEFITS AND
CONSTRUCTI LOADS
PRODUCT STAGE ON PROCESS USE STAGE END OF LIFE STAGE BEYOND THE
STAGE SYSTEM
BOUNDARIES
7 Environmental Product Declaration Hilti AG – HVU2
lairetam
waR
ylppus tropsnarT
gnirutcafunaM
eht
morf
tropsnarT
etis
eht
ot
etag
ylbmessA esU
ecnanetniaM
riapeR
tnemecalpeR tnemhsibrufeR
ygrene
lanoitarepO esu
retaw
lanoitarepO esu
noitcurtsnoc­eD
noitilomed tropsnarT
gnissecorp
etsaW
lasopsiD ­esueR ­yrevoceR ­gnilcyceR laitnetop
A1 A2 A3 A4 A5 B1 B2 B3 B4 B5 B6 B7 C1 C2 C3 C4 D
X X X X X ND ND MNR MNR MNR ND ND X X X X X
RESULTS OF THE LCA - ENVIRONMENTAL IMPACT according to EN 15804+A2: 1 kg HVU2
Core Indicator Unit A1 A2 A3 A4 A5 C1 C2 C3 C4 D
GWP­total [kg CO2­Eq.] 2.05E+0 4.28E­2 5.25E­1 7.62E­2 1.19E­1 4.02E­3 4.98E­3 0.00E+0 1.18E­1 0.00E+0
GWP­fossil [kg CO2­Eq.] 2.03E+0 4.27E­2 4.06E­1 7.59E­2 1.06E­1 4.02E­3 4.96E­3 0.00E+0 1.17E­1 0.00E+0
GWP­biogenic [kg CO2­Eq.] 2.09E­2 1.28E­4 1.18E­1 2.64E­4 1.21E­2 3.65E­6 1.72E­5 0.00E+0 2.94E­4 0.00E+0
GWP­luluc [kg CO2­Eq.] 1.10E­3 2.03E­5 1.27E­3 3.03E­5 2.45E­4 4.00E­7 1.98E­6 0.00E+0 2.21E­6 0.00E+0
ODP [kg CFC11­Eq.] 3.41E­7 9.66E­9 9.33E­8 1.76E­8 5.73E­9 8.59E­10 1.15E­9 0.00E+0 3.20E­9 0.00E+0
AP [mol H+­Eq.] 9.13E­3 2.89E­4 1.83E­3 2.16E­4 6.03E­4 4.17E­5 1.41E­5 0.00E+0 7.86E­5 0.00E+0
EP­freshwater [kg P­Eq.] 6.44E­4 2.73E­6 1.40E­4 5.19E­6 1.14E­4 1.27E­7 3.39E­7 0.00E+0 8.84E­7 0.00E+0
EP­marine [kg N­Eq.] 1.96E­3 6.30E­5 7.71E­4 4.40E­5 1.05E­4 1.85E­5 2.88E­6 0.00E+0 2.20E­3 0.00E+0
EP­terrestrial [mol N­Eq.] 1.78E­2 6.96E­4 4.75E­3 4.78E­4 9.14E­4 2.03E­4 3.12E­5 0.00E+0 3.16E­4 0.00E+0
POCP [kg NMVOC­Eq.] 6.14E­3 2.11E­4 1.21E­3 1.84E­4 2.51E­4 5.57E­5 1.20E­5 0.00E+0 1.15E­4 0.00E+0
ADPE [kg Sb­Eq.] 2.03E­5 1.42E­7 1.83E­6 2.74E­7 9.83E­7 2.04E­9 1.79E­8 0.00E+0 3.20E­8 0.00E+0
ADPF [MJ] 3.51E+1 6.20E­1 6.32E+0 1.13E+0 2.28E+0 5.41E­2 7.39E­2 0.00E+0 2.29E­1 0.00E+0
[m³ world­Eq
WDP 1.10E+0 2.80E­3 2.48E­1 5.29E­3 6.12E­2 1.45E­4 3.46E­4 0.00E+0 2.37E­3 0.00E+0
deprived]
GWP = Global warming potential; ODP = Depletion potential of the stratospheric ozone layer; AP = Acidification potential of land and water; EP =
Caption Eutrophication potential; POCP = Formation potential of tropospheric ozone photochemical oxidants; ADPE = Abiotic depletion potential for non­
fossil resources; ADPF = Abiotic depletion potential for fossil resources; WDP = Water (user) deprivation potential
RESULTS OF THE LCA - INDICATORS TO DESCRIBE RESOURCE USE according to EN 15804+A2: 1 kg
HVU2
Indicator Unit A1 A2 A3 A4 A5 C1 C2 C3 C4 D
PERE [MJ] 1.22E+0 8.49E­3 5.50E­1 1.64E­2 4.55E­1 3.09E­4 1.07E­3 0.00E+0 1.21E­2 0.00E+0
PERM [MJ] 4.58E­2 0.00E+0 1.58E+0 0.00E+0 0.00E+0 0.00E+0 0.00E+0 0.00E+0 0.00E+0 0.00E+0
PERT [MJ] 1.27E+0 8.49E­3 2.13E+0 1.64E­2 4.55E­1 3.09E­4 1.07E­3 0.00E+0 1.21E­2 0.00E+0
PENRE [MJ] 2.92E+1 6.20E­1 5.06E+0 1.13E+0 2.28E+0 5.41E­2 7.39E­2 0.00E+0 2.29E­1 0.00E+0
PENRM [MJ] 5.89E+0 0.00E+0 1.26E+0 0.00E+0 0.00E+0 0.00E+0 0.00E+0 0.00E+0 0.00E+0 0.00E+0
PENRT [MJ] 3.51E+1 6.20E­1 6.32E+0 1.13E+0 2.28E+0 5.41E­2 7.39E­2 0.00E+0 2.29E­1 0.00E+0
SM [kg] 1.04E­2 2.28E­4 1.91E­1 3.85E­4 2.39E­4 2.12E­5 2.51E­5 0.00E+0 8.67E­5 0.00E+0
RSF [MJ] 5.18E­4 2.14E­6 1.37E­2 4.23E­6 1.96E­6 6.91E­8 2.77E­7 0.00E+0 3.95E­6 0.00E+0
NRSF [MJ] 0.00E+0 0.00E+0 0.00E+0 0.00E+0 0.00E+0 0.00E+0 0.00E+0 0.00E+0 0.00E+0 0.00E+0
FW [m³] 2.73E­2 7.47E­5 5.88E­3 1.44E­4 1.92E­3 3.28E­6 9.42E­6 0.00E+0 3.00E­4 0.00E+0
PERE = Use of renewable primary energy excluding renewable primary energy resources used as raw materials; PERM = Use of
renewable primary energy resources used as raw materials; PERT = Total use of renewable primary energy resources; PENRE = Use of
non­renewable primary energy excluding non­renewable primary energy resources used as raw materials; PENRM = Use of non­
Caption
renewable primary energy resources used as raw materials; PENRT = Total use of non­renewable primary energy resources; SM = Use
of secondary material; RSF = Use of renewable secondary fuels; NRSF = Use of non­renewable secondary fuels; FW = Use of net fresh
water
RESULTS OF THE LCA – WASTE CATEGORIES AND OUTPUT FLOWS according to EN 15804+A2:
1 kg HVU2
Indicator Unit A1 A2 A3 A4 A5 C1 C2 C3 C4 D
HWD [kg] 7.43E­1 7.43E­4 2.98E­2 1.29E­3 8.03E­3 7.23E­5 8.40E­5 0.00E+0 3.57E­4 0.00E+0
NHWD [kg] 1.66E+0 1.20E­2 4.08E­1 2.28E­2 5.06E­1 5.08E­4 1.49E­3 0.00E+0 1.03E+0 0.00E+0
RWD [kg] 5.34E­5 4.28E­6 1.35E­5 7.78E­6 1.67E­5 3.81E­7 5.08E­7 0.00E+0 1.52E­6 0.00E+0
CRU [kg] 0.00E+0 0.00E+0 0.00E+0 0.00E+0 0.00E+0 0.00E+0 0.00E+0 0.00E+0 0.00E+0 0.00E+0
MFR [kg] 6.97E­4 1.29E­5 5.00E­2 3.54E­6 2.16E­1 7.20E­8 2.31E­7 0.00E+0 1.25E­6 0.00E+0
MER [kg] 3.06E­6 1.59E­8 7.68E­7 2.85E­8 1.77E­8 1.15E­9 1.86E­9 0.00E+0 6.02E­9 0.00E+0
EEE [MJ] 1.04E­2 1.28E­4 1.30E­2 2.46E­4 4.33E­3 2.12E­5 1.61E­5 0.00E+0 4.67E­4 0.00E+0
EET [MJ] 4.06E­2 5.93E­4 3.62E­2 1.02E­3 1.42E­2 2.15E­4 6.69E­5 0.00E+0 1.26E­3 0.00E+0
HWD = Hazardous waste disposed; NHWD = Non­hazardous waste disposed; RWD = Radioactive waste disposed; CRU = Components
Caption for re­use; MFR = Materials for recycling; MER = Materials for energy recovery; EEE = Exported electrical energy; EEE = Exported
thermal energy
RESULTS OF THE LCA – additional impact categories according to EN 15804+A2-optional:
1 kg HVU2
Indicator Unit A1 A2 A3 A4 A5 C1 C2 C3 C4 D
[Disease
PM 7.61E­8 3.12E­9 2.44E­8 6.12E­9 2.11E­9 1.12E­9 4.00E­10 0.00E+0 1.67E­9 0.00E+0
Incidence]
[kBq U235­
IRP 1.25E­1 3.20E­3 3.07E­2 5.93E­3 6.15E­2 2.48E­4 3.88E­4 0.00E+0 1.52E­3 0.00E+0
Eq.]
ETP­fw [CTUe] 7.39E+1 5.04E­1 5.75E+0 9.43E­1 1.54E+0 3.25E­2 6.16E­2 0.00E+0 4.97E­1 0.00E+0
HTP­c [CTUh] 7.73E­9 1.83E­11 1.77E­10 2.90E­11 5.03E­11 1.25E­12 1.89E­12 0.00E+0 7.33E­12 0.00E+0
HTP­nc [CTUh] 1.34E­7 4.76E­10 3.84E­9 9.23E­10 1.65E­9 2.35E­11 6.03E­11 0.00E+0 1.86E­10 0.00E+0
SQP [­] 4.47E+0 3.95E­1 8.66E+0 8.02E­1 4.22E­1 7.03E­3 5.25E­2 0.00E+0 6.00E­1 0.00E+0
PM = Potential incidence of disease due to PM emissions; IR = Potential Human exposure efficiency relative to U235; ETP­fw = Potential
Caption comparative Toxic Unit for ecosystems; HTP­c = Potential comparative Toxic Unit for humans (cancerogenic); HTP­nc = Potential
comparative Toxic Unit for humans (not cancerogenic); SQP = Potential soil quality index
Disclaimer 1 – for the indicator “Potential Human exposure efficiency relative to U235”.
This impact category deals mainly with the eventual impact of low dose ionizing
radiation on human health of the nuclear fuel cycle. It does not consider effects due to possible
nuclear accidents, occupational exposure nor due to radioactive waste disposal in underground
facilities. Potential ionizing radiation from the soil, from radon and from some construction materials is also not
measured by this indicator.
Disclaimer 2 – for the indicators “abiotic depletion potential for non­fossil resources”, “abiotic depletion potential
for fossil resources”, “water (user) deprivation potential, deprivation­weighted water consumption”, “potential
comparative toxic unit for ecosystems”, “potential comparative toxic unit for humans – cancerogenic”, “Potential
comparative toxic unit for humans ­ not cancerogenic”, “potential soil quality index”.
The results of this environmental impact indicator shall be used with care as the
uncertainties on these results are high or as there is limited experienced with the indicator.
6. LCA: Interpretation
The dominance analysis shows that the main causes composition, cause a little bit less than 50% of the
of environmental impacts and indicators can be found module’s impact regarding global warming.
in the information module A1. This shows the global
warming potential for the provision of material with
about 70%, based on all information modules. Module
A3 also represents an import part of the final impact
Illustration: Dominance analysis A1
The mass of the individual components of the resin
mixture and mineral fillers come from the recipe
information provided by the manufacturer. According to
Illustration: Dominance analysis A1- C4
the manufacturer, this information can be assumed to
be highly accurate.
Module A1 is detailed below. Module A3’s global
warming impact is mostly constituted by the final
The relevant datasets used to calculate the material
product packaging (12% of the total impact) and the
availability of the product are highly topical since the
energy used for manufacturing (4% of the total impact).
raw materials were detailed as much as necessary to
find corresponding data in the latest Ecoinvent
In the information module A1, the material supply of
database (2021). The locations were also respected.
the resin mixture causes more than 50% of the global
Since these datasets strongly influence the results, as
warming potential. The mineral fillers, which represent
shown by the dominance analysis, so does the overall
the raw materials with the most import part in the
computation.
7. Requisite evidence
Hilti HVU2 complies with the requirements of  emission class A+ outlined in the French VOC
 DIBt (2010) in combination with the NIK Directives (2017) in accordance with the
values from AgBB (2015) for applications in Eurofins attestation,
interior areas,  CDPH/EHLB Standard Method V 1.2 (2017)
8 Environmental Product Declaration Hilti AG – HVU2
in accordance with Eurofins test report, No. 392-2017- Sum SVOC (C16 ­ C22) <100 μg/m3
00087601_D_EN, Eurofins test report, No. 392-2017- R (dimensionless) <1 ­
00087601_E_EN and Eurofins test report, No. 392- VOC without NIK <100 μg/m3
2017-00087601_H_EN respectively. Carcinogenic Substances <1 μg/m3
AgBB overview of results (3 days [µg/m³])
Name Value Unit
AgBB overview of results (28 days [µg/m³]) VOC without NIK <10000 μg/m3
Name Value Unit Carcinogenic Substances <10 μg/m3
TVOC (C6 ­ C16) <1000 μg/m3
8. References
Standards Institut Bauen und Umwelt e.V, Berlin (pub.): Product
Category Rules for Construction Products from the
DIN EN 13501-1 range of Environmental Product Declarations for
Klassifizierung von Bauprodukten und Bauarten zu Institut Bauen und Umwelt (IBU), Part A: Calculation
ihrem Brandverhalten Rules for the Life Cycle Assessment and
Requirements on the Project Report according to EN
15804+A2:2019, 2021­04
DIN EN 14293
Klebstoffe ­ Klebstoffe für das Kleben von Parkett auf PCR Part B
einen Untergrund ­ Prüfverfahren und Institut Bauen und Umwelt e.V, Berlin (pub.): Product
Mindestanforderungen Category Rules for Construction Products from the
range of Environmental Product Declarations for
Institut Bauen und Umwelt (IBU), Part B: Requirements
DIN EN ISO 50001 on the EPD for Reaction resin products, 2019­01
DIN EN ISO 50001: 2018 Energy management
systems ­ Requirements with guidance for use
Further References
EN 15804
EN 15804:2012+A1:2013, Sustainability of AFNOR, «FD P01-015» 2006
construction works — Environmental Product Qualité environnementale des produits de construction
Declarations — Core rules for the product category of ­ Fascicule de données énergie et transport
construction products.
AgBB (2015)
EN 15804 Vorgehensweise bei der gesundheitlichen Bewertung
EN 15804:2012+A2:2019, Sustainability of der Emissionen von flüchtigen organischen
construction works — Environmental Product Verbindungen (VVOC, VOC und SVOC) aus
Declarations — Core rules for the product category of Bauprodukten (2018)
construction products.
Candidate List of substances of very high concern
EN ISO 604 for Authorisation
DIN EN ISO 604:2003­12: Determination of European Cheminals Agency (ECHA), in accordance
compressive properties with Article 50(10) of the REACH regulation
EN ISO 1183-1 CDPH/EHLB/Standard Method V1.2
DIN 51757:2011­01 Plastics ­ Methods for determining California CDPH Standard Method is a US standard for
the density of non­cellular plastics ­ Part 1: Immersion evaluating and restricting VOC emissions to indoor air.
method, liquid pyknometer method and titration Developed in California as "Section 01350"
method Specification, several systems in the US refer to CDPH
Standard Method
Comité National Routier (CNR)
ISO 9001 Enquête longue distance, PARIS, 2019
ISO 9001:2015 Quality management systems ­
Requirements DIBt (2010)
Grundsätze zur gesundheitlichen Bewertung von
Bauprodukten in Innenräumen (Oktober 2010)
ISO 14001 Eurofins test report, No. 392­2019­00435401_D_EN
ISO 14001:2015 Environmental management systems VOC test report for verification of compliance with
­ Requirements with guidance for use DIBt(2010)/AgBB(2018)
ISO 14025 Eurofins test report, No. 392-2017-00087601_D_EN
EN ISO 14025:2011, Environmental labels and VOC test report for verification of compliance with
declarations — Type III environmental declarations — DIBt(2010)/AgBB(2015)
Principles and procedures.
Eurofins test report, No. 392-2017-00087601_E_EN
PCR Part A VOC test report for verification of compliance with the
9 Environmental Product Declaration Hilti AG – HVU2
French VOC directive from 2017 Umwelt Bundesamt: Herkunftsnachweisregister
(HKNR) — Entwertungsnachweis durch GETECH
Eurofins test report, No. 392-2017-00087601_H_EN ENERGIE GMBH für HILTI
VOC test report for verification of compliance with
CDPH/EHLB/Standard Method V1.2 from 2017
European Waste code Database
in accordance with the European Waste Catalogue
(EWC) (EWC 2014/955/EU) Commission Decision Ecoinvent 3.8
amending Decision 2000/532/EC on the list of waste ecoinvent Version 3
pursuant to Directive 2008/98/EC of the European Wernet, G., Bauer, C., Steubing, B., Reinhard, J.,
Parliament and of the Council Moreno­Ruiz, E., and Weidema, B., 2016. The
ecoinvent database version 3 (part I): overview and
ETA 16/0515 methodology. The International Journal of Life Cycle
European Technical Approval Hilti HVU2 Assessment, [online] 21(9), pp.1218–1230. Available
at: <http://link.springer.com/10.1007/s11367­016­1087­
French VOC Directives 8> [Accessed in 2021/2022].
Décret no 2011­321 du 23 mars 2011 relatif à
l’étiquetage des produits de construction ou de
revêtement de mur ou de sol et des peintures et vernis
sur leurs émissions de polluants volatils Publication
Arrêté du 19 avril 2011 relatif à l’étiquetage des
produits de construction ou de revêtement de mur ou IBU 2021
de sol et des peintures et vernis sur leurs émissions de Institut Bauen und Umwelt e.V.: General Instructions
polluants volatils for the EPD programme of Institut Bauen und Umwelt
e.V., Version 2.0, Berlin: Institut Bauen und Umwelt
NSF e.V., 2021
NSF/ANSI/CAN 61 Drinking Water System www.ibu­epd.com
Components ­ Health Effects
Umwelt Bundesamt 2021
10 Environmental Product Declaration Hilti AG – HVU2
Publisher
Institut Bauen und Umwelt e.V. Tel +49 (0)30 3087748­ 0
Hegelplatz 1 Fax +49 (0)30 3087748­ 29
10117 Berlin Mail info@ibu­epd.com
Germany Web www.ibu-epd.com
Programme holder
Institut Bauen und Umwelt e.V. Tel +49 (0)30 ­ 3087748­ 0
Hegelplatz 1 Fax +49 (0)30 – 3087748 ­ 29
10117 Berlin Mail info@ibu­epd.com
Germany Web www.ibu-epd.com
Author of the Life Cycle
Assessment Tel +33 (0)9 53 23 98 30
ESTEANA Fax ­
Rue Mège 26 Mail contact@esteana.fr
83220 Le Pradet Web www.esteana.fr
France
Owner of the Declaration
Hilti Aktiengesellschaft Tel +423 234 2111
Feldkircher Strasse 100 Fax +423 234 2965
9494 Schaan Mail HAGHSE@hilti.com
Liechtenstein Web www.hilti.com
