ver1 2015
ENVIRONMENTAL PRODUCT DECLARATION
in accordance with ISO 14025, ISO 21930 and EN 15804
Owner of the declaration: Hydro Aluminium AS
Program operator: The Norwegian EPD Foundation
Publisher: The Norwegian EPD Foundation
Declaration number: NEPD-2265-1034-EN
Registration number: NEPD-2265-1034-EN
ECO Platform reference number: -
Issue date: 18.06.2020
Valid to: 18.06.2025
Hydro Aluminium Primary Foundry Alloys Europe
Si content > 8%
Hydro Aluminium AS
www.epd-norge.no
NEPD-2265-1034-EN Hydro Aluminium Primary Foundry Alloys Europe Si content > 8%
General information
Product: Owner of the declaration:
Hydro Aluminium Primary Foundry Alloys Europe, Si content Hydro Aluminium AS
>8% Contact person: Leonhard Heusler
Phone: +49 2285522217
e-mail: Leonhard.heusler@hydro.com
Program operator: Manufacturer:
The Norwegian EPD Foundation Hydro Alumium AS
Pb. 5250 Majorstuen, 0303 Oslo Drammensveien 263, N-0240 Oslo
Phone: +47 97722020 Phone: +47 22538100
e-mail: post@epd-norge.no e-mail: greener@hydro.com
Declaration number: Place of production:
NEPD-2265-1034-EN Hydro Aluminium Sunndal
Hydro Aluminium Årdal
Slovalco
ECO Platform reference number: Management system:
IATF 16949, ISO 9001:2016, ISO 14001,
ISO 45001, ISO 50001
This declaration is based on Product Category Rules: Organisation no:
CEN Standard EN 15804 serves as core PCR 917 537 534
NPCR 013, "Version 3.0 Part B for steel and aluminium
construction products"
Statement of liability: Issue date:
The owner of the declaration shall be liable for the 18.06.2020
underlying information and evidence. EPD Norway shall
not be liable with respect to manufacturerinformation, life Valid to:
cycle assessment data and evidences. 18.06.2025
Declared unit: Year of study:
1 kg Hydro Aluminium Primaru Foundry Alloy Europe, Si 2020
content >8%
Declared unit with option: Comparability:
1 kg Hydro Aluminium Primary Foundry Alloy Europe, Si EPD of construction products may not be comparable if they
content >8% , including waste handling and possible not comply with EN 15804 and seen in a building context.
environmental benefits after end of life.
Functional unit: The EPD has been worked out by:
The product is an input to automotive parts and to different Irmeline de Sadeleer, Andreas Brekke, Kari-Anne Lyng
building and construction products. No use scenarios are
defined, hence no functional unit.
Verification:
The CEN Norm EN 15804 serves as the core PCR.
Independent verification of the declaration and data,
according to ISO14025:2010
internal external
Approved
Third party verifier:
sign
Jane Anderson, ConstructionLCA Limited
(Independent verifier approved by EPD Norway)
NEPD-2265-1034-EN Hydro Aluminium Primary Foundry Alloys Europe Si content > 8% 2/8
Product
Product description: Technical data:
This EPD covers production of Primary Foundry Alloys from All alloys meet specifications in accordance with relevant
Hydro Aluminium's European Smelters with alloy content > 8% ISO, EN and JIS standards.
Consistent high metal quality is ensured by using top-grade Alloys are produced as continuous cast or mold cast
raw materials, standardized production processes and ingots. The products are stacked and strapped into
continuous quality control. bundles of various sizes. Depending on the particular
production source, our foundry alloy ingots are supplied
in weights of 7-22 kg, and bundle weights can range
Product specification:
from 700-1200 kg.
Materials kg % For more detailed information on our products:
Primary Liquid Al from own Electrolysis 0.85-0.9 85-90% https://www.hydro.com/en-NO/products-and-
Primary Metal from external sources 0.01-0.03 1-3% services/casthouse-products/foundry-alloys/
Alloying Elements 0.08-0.12 8-12%
Examples of Industry we serve: Reference service life, product:
Automotive (Wheels, Chassis & Engine parts), Electrical Dependent on product application, but the material itself
applications, decorative / anodized applications has an infinite life time.
Market: Reference service life, building:
European Automotive & non automotive market for cast parts Dependent on product application, but the material itself
has an infinite life time.
NEPD-2265-1034-EN Hydro Aluminium Primary Foundry Alloys Europe Si content > 8% 3/8
LCA: Calculation rules
Declared unit: System boundary:
1 kg Hydro Aluminium Primary Foundry Alloys Europe Si Cradle to gate with options. The following stages have been
content >8%. The EPD also covers modules C2-C4 and D. declared: A1-A4, C2-C4 and D. Further specified in flow
sheet below.
The foundry alloys are produced in three smelters: Sunndal
and Årdal in Norway, and Slovalco in Slovakia. The
Module D covers the potential benefits from recycling of
presented results is a weighed average of production
Hydro Aluminium Foundry Alloy after end of useful life.
volumes in 2017.
Module D covers all necessary stages from C3 until the
aluminium is back on the market and compares to the
environmental performance of an average market foundry
alloy. The module is further specified under scenarios.
Data quality: Cut-off criteria:
Specific data are used for all of Hydro's processes, based on the All major raw materials and all the essential energy is
production year 2017, and are collected the first months of 2019. included. The production process for raw materials and
As Hydro has ownership in a total value chain from mining of energy flows that are included with very small amounts
bauxite to production of aluminium extrusion ingots, all stages (<1%) are not included. This cut-off rule does not apply for
from A1 to A4 are covered by specific data. Background data on hazardous materials and substances, and mostly apply for
for instance transport and electricity production are from alloying elements that are added in less than per
ecoinvent 3.4 (April 2018). thousandth.
Allocation:
The allocation is made in accordance with the provisions of
EN 15804. Incoming energy and water and waste production
inhouse is allocated equally among all products through
mass allocation. For almost all processes, detailed data are
provided for each process step, and the main allocation is
between aluminium hydroxide and aluminium oxide in the
production of alumina. Effects of primary production of
recycled materials are allocated to the main product in which
the material was used. The recycling process and
transportation of the material is allocated to this analysis.
NEPD-2265-1034-EN Hydro Aluminium Primary Foundry Alloys Europe Si content > 8% 4/8
LCA: Scenarios and additional technical information
The following information describe the scenarios in the different modules of the EPD.
The transport from production sites to market is assumed to be the weighted distance from the two smelters in Norway and the
one in Slovakia to a location in central Europe.
Transport from production place to user (A4)
Type Capacity utilisation Type of vehicle Distance km Fuel/Energy
(incl. return) % consumption
Truck 50 Lorry, >32 metric tons, Euro V 611 2.46 E-02 l/tkm
Boat 80 Cargo ship, 5000 tons 1019 1.56 E-02 l/tkm
Most of the aluminium used for construction purposes is collected (approximately 96%) and recycled (approximately
97% of the collected aluminium), giving a total of 93% recycled. The aluminium is transported to a material
processing site where different materials, including metals are shredded and sorted. Most of the aluminium used in
the automotive industry is collected (approximately 95%) and recycled (approximately 97% of the collected
aluminium), giving a total of 92% recycled. The rest is assumed landfilled.
End of Life (C2, C3, C4)
Unit Value
Hazardous waste disposed kg -
Collected kg 0.951
Reuse kg -
Recycling kg 0.924
Energy recovery kg 0.027*
To landfill kg 0.049**
*27 grams of the original 1 kg of aluminium is going to incineration. No loads or beneifts are attribuded to this flow.
**There will be a small portion of aluminium ending as uncollected. This is included under "To landfill" where no loads or benefits are included.
Transport to waste processing (C2)
Type Capacity utilisation Type of vehicle Distance km Fuel/Energy
Truck 40 Lorry, >32 metric tons, Euro V 50 2.85 E-02 l/tkm
Aluminium from construction site to waste handling site is assumed to be transported in an older medium-sized lorry with
smaller capacity utilization than in the production system
Benefits and loads beyond the system boundaries (D)
Unit Value
Aluminium foundry alloy to recycling g 924
Aluminium collected and recycled is assumed to replace an average extrusion ingot in Europe consisting of 40% recycled
and 60% primary aluminium. This is a conservative approach.
NEPD-2265-1034-EN Hydro Aluminium Primary Foundry Alloys Europe Si content > 8% 5/8
LCA: Results
System boundaries (X=included, MND= module not declared, MNR=module not relevant)
Environmental impact
Resource use
noitilomed
noitcurtsnoc-eD
MND
tnemecalpeR
B5
kg CFC11-eqv
1.97E-05
4.72E-04 6.97E-04 0.00E+00
tnemhsibrufeR
3.04E-05
ecnanetniaM
esu
retaw
lanoitarepO
A1 A5
x
7.78E-03
ODP 4.21E-07
ylbmessA
x MND
A4 C2
riapeR
0.00E+00
7.15E-05
1.07E-07
MJ
MJ
0.00E+00
TRPE MJ 5.38E+01
SM kg
RSF MJ 0.00E+00
MJ 0.00E+00
m3 6.08E-02
esU
End of life stage
B1
kg CO -eqv
2
2.75E-02
kg PO 3--eqv 4
tropsnarT
C2
Parameter
tropsnarT
x
gnirutcafunaM
Product stage Assemby stage
x
tropsnarT
A2
MND MND MND
slairetam
waR
A3 A4 B3 D
MND
A1-A3 C3
6.99E-02 -4.87E+00
9.63E-09 -2.98E-07
1.33E-03 0.00E+00 -2.61E-03
-3.10E-02
0.00E+00 -1.62E-03
-1.22E-05
0.00E+00 -4.71E+01
D
0.00E+00
0.00E+00
-2.29E+01
-5.72E+01
0.00E+00
-5.72E+01
0.00E+00
0.00E+00 0.00E+00
0.00E+00 0.00E+00
0.00E+00 -4.36E-02
lasopsiD
-gnilcyceR-yrevoceR-esueR
laitnetop
C4
x
gnissecorp
etsaW
All results are calculated with the use of SimaPro v.9 (2019) and impact methods according to ISO 15804. Results are based on a
weighted average between three production sites.
Beyond the
system
boundaries
B2 B4 B6 B7 C1 C3
x MND MND MND x x
Unit C4 D
GWP 4.95E+00 2.48E-01
1.92E-08 1.44E-09 0.00E+00
AP kg SO 2 -eqv 3.05E-05
EP 8.73E-03 5.47E-06
ADPM kg Sb-eqv 9.95E-06 2.35E-08 0.00E+00
MJ 4.56E+01 1.63E+00 1.35E+00
GWP Global warming potential; ODP Depletion potential of the stratospheric ozone layer; POCP Formation potential of tropospheric
photochemical oxidants; AP Acidification potential of land and water; EP Eutrophication potential; ADPM Abiotic depletion potential for non
fossil resources; ADPE Abiotic depletion potential for fossil resources
Unit A1-A3 A4 C3 C4
RPEE MJ 5.11E+01 1.25E-02 1.72E-01 -2.29E+01
RPEM 0.00E+00 0.00E+00 0.00E+00 0.00E+00 0.00E+00
TPE 5.11E+01 1.25E-02 1.19E-03 1.72E-01 0.00E+00
NRPE MJ 5.38E+01 1.57E+00 1.20E-01 1.52E+00 0.00E+00
NRPM MJ 0.00E+00 0.00E+00 0.00E+00 0.00E+00
1.57E+00 1.20E-01 1.52E+00 0.00E+00
0.00E+00 0.00E+00 0.00E+00 0.00E+00
0.00E+00 0.00E+00
NRSF 0.00E+00 0.00E+00
W 2.69E-04 2.25E-05
RPEE Renewable primary energy resources used as energy carrier; RPEM Renewable primary energy resources used as raw materials;
TPE Total use of renewable primary energy resources; NRPE Non renewable primary energy resources used as energy carrier; NRPM Non
renewable primary energy resources used as materials; TRPE Total use of non renewable primary energy resources; SM Use of secondary
materials; RSF Use of renewable secondary fuels; NRSF Use of non renewable secondary fuels; W Use of net fresh water
esu
ygrene
lanoitarepO
Use stage
POCP kg C 2H 4 -eqv 1.29E-06
1.59E-04
1.64E-06
ADPE 1.25E-01
Parameter C2
1.19E-03
0.00E+00
0.00E+00
0.00E+00
7.37E-04
NEPD-2265-1034-EN Hydro Aluminium Primary Foundry Alloys Europe Si content > 8% 6/8
End of life - Waste
Parameter Unit A1-A3 A4 C2 C3 C4 D
HW kg 2.05E-02 7.34E-07 7.61E-08 6.11E-03 0.00E+00 4.91E-03
NHW kg 3.36E+00 8.13E-02 6.36E-03 1.15E+00 9.80E-02 -2.49E+00
RW kg 2.71E-04 1.08E-05 8.12E-07 4.81E-06 0.00E+00 -2.26E-04
HW Hazardous waste disposed; NHW Non hazardous waste disposed; RW Radioactive waste disposed
End of life - Output flow
Parameter Unit A1-A3 A4 C2 C3 C4 D
CR kg - - - - - -
MR kg - - - 9.25E-01 - -
MER kg - - - 2.57E-02 - -
EEE MJ - - - - - -
ETE MJ - - - - - -
CR Components for reuse; MR Materials for recycling; MER Materials for energy recovery; EEE Exported electric energy; ETE Exported
thermal energy
Reading example: 9.0 E-03 = 9.0*10-3 = 0.009
Additional Norwegian requirements
Greenhouse gas emission from the use of electricity in the manufacturing phase
National production mix from import, low voltage (production of transmission lines, in addition to direct emissions and losses in
grid) of applied electricity for the manufacturing process (A3).
Data source Amount Unit
ecoinvent v3.4 (April 2018) 4 g CO -eqv/kWh
2
Dangerous substances
The product contains no substances given by the REACH Candidate list or the Norwegian priority list
The product contains substances given by the REACH Candidate list or the Norwegian priority list that are less than 0.1 %
by weight.
The product contain dangerous substances, more than 0.1% by weight, given by the REACH Candidate List or the
Norwegian Priority list, see table.
The product contains no substances given by the REACH Candidate list or the Norwegian priority list. The product is
classified as hazardous waste (Avfallsforskiften, Annex III), see table.
Name CAS no. Amount
Indoor environment
Not relevant
Carbon footprint
Calculations connected to climate change and global warming potential (GWP) include greenhouse gas emissions from fossil
sources and land use change connected to extraction of bauxite, but does not include calculations of biogenic emissions of CO .
2
NEPD-2265-1034-EN Hydro Aluminium Primary Foundry Alloys Europe Si content > 8% 7/8
Bibliography
ISO 14025:2010 Environmental labels and declarations - Type III environmental declarations - Principles
and procedures
ISO 14044:2006 Environmental management - Life cycle assessment - Requirements and guidelines
EN 15804:2012+A1:2013 Sustainability of construction works - Environmental product declaration - Core rules for
the product category of construction products
ISO 21930:2007 Sustainability in building construction - Environmental declaration of building products
NPCR 013 NPCR 013 version 3.0 Part B for steel and aluminium construction products.
Sadeleer, I., Brekke, A. and Background report for the Environmental Product Declarations for Hydro Aluminium
Lyng, Kari-Anne (2020) Wire Rod, Hydro Aluminium Sheet Ingot and Hydro Aluminium Foundry Alloy
Program operator Phone: +47 97722020
The Norwegian EPD Foundation
Post Box 5250 Majorstuen, 0303 Oslo e-mail: post@epd-norge.no
Norway web www.epd-norge.no
Publisher Phone: +47 97722020
The Norwegian EPD Foundation
Post Box 5250 Majorstuen, 0303 Oslo e-mail: post@epd-norge.no
Norway web www.epd-norge.no
Owner of the declaration Phone: +49 2285522217
Hydro Aluminium AS Fax
Drammensveien 263 e-mail: Leonhard.heusler@hydro.com
N-0240 Oslo web www.hydro.com
Author of the Life Cycle Assessment Phone: +47 69 35 11 00
Østfoldforskning Fax +47 69 34 24 94
Company logo
Stadion 4 e-mail: post@ostfoldforskning.no
1671 Kråkerøy web www.ostfoldforskning.no
NEPD-2265-1034-EN Hydro Aluminium Primary Foundry Alloys Europe Si content > 8% 8/8
