ENVIRONMENTAL PRODUCT DECLARATION
as per ISO 14025 and EN 15804+A2
Owner of the Declaration Holcim (Romania) SA
Programme holder Institut Bauen und Umwelt e.V. (IBU)
Publisher Institut Bauen und Umwelt e.V. (IBU)
Declaration number IBU-CEI-HOL-2205120-RO2025000049-ISUE001-EN
Issue date 26/02/2025
Valid to 25/02/2030
Concrete ECOPact C20/25Cl02D16S3 produced in plant
RMX Timisoara 1
Mix code 833290, EPD Version 1
Holcim (Romania) SA
www.ibu-epd.com | https://epd-online.com
1. General Information
Holcim (Romania) SA ECOPact C20/25Cl02D16S3
Programme holder Owner of the declaration
IBU - Institut Bauen und Umwelt e.V. Holcim (Romania) SA
Hegelplatz 1 46D-46E-48, Pipera Road, Oregon Park - Building B,
10117 Berlin 6th Floor
Germany 020309 Bucharest
Romania
Declaration number Declared product / Declared unit
IBU-CEI-HOL-2205120-RO2025000049-ISUE001-EN 1 m3 of unreinforced concrete ECOPact
C20/25Cl02D16S3
This declaration is based on the product Scope:
category rules: This document refers to the production of
Concrete components made of in-situ or ready- ECOPact C20/25Cl02D16S3 concrete, mix
mixed concrete, 03.2022 (PCR checked and code 833290 produced in the plant of RMX
approved by the SVR) Timisoara 1 of Holcim (Romania) SA in Romania
for use as concrete in building construction and
Issue date civil engineering.
26/02/2025
The EPD was calculated with the pre-verified
Valid to software CarbonCLARITYTM EN 15804 EPD
25/02/2030 Generator - RMX of Climate Earth.
The owner of the declaration shall be liable for
the underlying information and evidence; the
IBU shall not be liable with respect to
manufacturer information, life cycle assessment
data and evidences.
The EPD was created according to the
specifications of EN 15804+A2. In the following,
the standard is simply referred to as EN 15804.
Verification
The standard EN 15804 serves as the core PCR
Independent verification of the declaration and data
according to ISO 14025:2011
Hans Peters internally x externally
(Chairman Institut Bauen und Umwelt e.V.)
Florian Pronold Matthias Schulz
(Managing Director Institut Bauen und Umwelt e.V.) (Independent verifier)
2 Environmental Product Declaration Holcim (Romania) SA – 833290 concrete, Plant RMX Timisoara 1
2. Product
2.1 Product description/Product definition 2.5 Base materials/Ancillary materials
Concrete is produced by mixing cement, aggregates Name Value Unit
and water with potentially additional cementitious Cement ca. 10-17 M.%
materials, fibers and additives.
Water ca. 7-10 M.%
Aggregate ca. 70-90 M.%
The fresh concrete is generally poured into formwork,
compacted and hardened in the desired form by Cementitious ca. <1 M.%
hydration of the cement to form a solid artificial rock. Fibers ca. <1 M.%
Admixtures ca. <1 M.%
The declared product is unreinforced concrete that is
delivered to the job site as ready-mix concrete. In the
case of reinforced components, the proportion of
reinforcing steel must be taken into account
separately.
To calculate the life cycle assessment of the ECOPact
C20/25Cl02D16S3 concrete in plant RMX Timisoara 1,
the production data from mix code 833290 were used.
For the use and application of the product the
respective national provisions at the place of use
apply, such as the building codes and the
corresponding national specifications.
2.2 Application
Concrete is a widely used building material in the
construction industry. It is used for example for the
construction of walls, stairs, floor, foundations, bored Note: dashed lines indicate production steps that do not
piles or even complete structures such as bridges. necessarily apply to this concrete
2.3 Technical data This product contains substances listed in the ECHA
Concrete ECOPact C20/25Cl02D16S3 has the candidate list (date: 14.06.2023) exceeding 0.1
following technical properties: percentage by mass: no
Technical data This product contains other CMR substances in
Name Value Unit categories 1A or 1B which are not on the candidate
Gross density 2314.74 kg/m3 list, exceeding 0.1 percentage by mass: no
Compressive
C20/25 N/mm2 Biocide products were added to this construction
strength
product or it has been treated with biocide products
(this then concerns a treated product as defined by the
This concrete product is produced according to (EU) Ordinance on Biocide Products No. 528/2012): no
standard EN 206:2013+A2:2021, Concrete -
Specification, performance, production and conformity 2.6 Manufacture
as a designed concrete. The dosed aggregates are first premixed with cement
as a binding agent and other additives. The mixture is
This technical data fulfill the requirements according to then mixed with water to form a plastically deformable
EN-206-1 standard regarding quality control and fresh concrete. This is transported to the customer
conformity checks. Testing is done according to EN where it is placed in the prepared formwork and
12350 and EN 12390. Further technical data, as compacted.
indicated in PCR B, are not relevant for this product.
This is because properties such as thermal To ensure the quality of the concrete, quality
conductivity, tensile strength or modulus of elasticity assurance systems is installed in RMX Timisoara 1
can be found in the regulations for the design of plant, which is based on the requirements for in-house
concrete components and are therefore not routinely production control in EN-206-1 standard.
checked.
2.7 Environment and health during manufacturing
Performance characteristics for fresh concrete in Fresh concrete and residual water recycling is
relation to its characteristics according to the relevant common practice in the RMX Timisoara 1 plant. Not
technical regulation (no CE marking). yet hardened concrete residues from mixers, concrete
vehicles, bucket conveyors and concrete distributors
2.4 Delivery status are washed out and both the aggregate and the
Fresh concrete is delivered to the customers in remaining water are reused as concrete raw materials.
concrete truck mixers. It can also be picked up by the
client using their trucks. Fresh concrete contains a strongly alkaline solution
that is created when cement is mixed with water and
3 Environmental Product Declaration Holcim (Romania) SA – 833290 concrete, Plant RMX Timisoara 1
can cause skin and eye irritation. The abrasiveness of According to EN 13501-1, concrete meets the
the aggregate used can also support this irritation. requirements of building material class A1, "non-
flammable". In the event of fire, no toxic gases and
Cements used within this product are low in chromate, vapors can arise, and burning concrete components do
as per requirements of REACH regulation, in order to not drip or fall off.
limit the development of allergic chromate dermatitis
that can happen in the event of prolonged contact with High fire resistance classes can be achieved through
the concrete. appropriate dimensioning of the components (in EN
1992-1-2 tabular values for fire resistance classes
Further information can be found in the safety data according to EN 13501-2 are given).
sheets.
holcim.ro Fire protection
Name Value
2.8 Product processing/Installation Building material class A1 "not combustible"
In general, after mixing the concrete is transported to
the construction site with trucks, placed in the prepared
Water
formwork by direct pouring or pumping and usually
When exposed to water (e.g. floods), concrete is
compacted with internal vibrators. After a sufficiently
largely inert. No substances are washed out in
long hardening time, the formwork is removed and the
quantities that could be hazardous to water.
concrete is cured further with time.
Mechanical destruction
2.9 Packaging
The mechanical destruction of concrete, e.g. by
The delivery of concrete does not require the use of
demolishing concrete, does not produce any
packaging material.
substances that are hazardous to the environment or
health.
2.10 Condition of use
The composition of the concrete does not
2.14 Re-use phase
fundamentally change when it is used.
Components made of concrete can be dismantled. The
concrete is first crushed and separated into individual
2.11 Environment and health during use
grain fractions and used in road construction or in
The natural ionizing radiation from concrete is low and
small proportions as recycled aggregate for the
harmless to health. The environmental compatibility of
production of fresh concrete. If steel fibers or rebar is
concrete is ensured by the fact that only standardized
included in the concrete, this is separated during or
starting materials may be used that are a priori
after demolition and reused as scrap. Recovery of
regarded as harmless.
alternative fibers or rebar is not commonplace.
2.12 Reference service life
2.15 Disposal
A reference service of 50 years is used for modeling
For construction waste made of concrete, the waste
concrete’s use phase.
codes 17 01 01 (concrete), 17 04 05 (steel fibers) and
17 02 03 (plastic fibers) (WCO) apply in accordance
2.13 Extraordinary effects
with the European list of waste.
Fire
2.16 Further information
Further information holcim.ro.
4 Environmental Product Declaration Holcim (Romania) SA – 833290 concrete, Plant RMX Timisoara 1
3. LCA: Calculation rules
3.1 Declared unit
1 m3 of unreinforced concrete ECOPact End of life
C20/25Cl02D16S3
Module C1: Dismantling /
In the case of reinforced components, the proportion of demolition of concrete buildings /
reinforcing steel must be taken into account components
separately.
Module C2: Transport of
Declared unit demolished concrete for processing
Designation Value unit
Declared unit 1 m3 Module C3: Concrete waste
processing
Density 2314.74 kg/m3
Conversion factor to 1 kg 4.32E-4 -
Module C4: Concrete waste
disposal
To calculate the life cycle assessment of the ECOPact
C20/25Cl02D16S3 concrete in plant RMX Timisoara 1, Module D
the production data from mix code 833290 were used.
Module D: Benefits and loads for
3.2 System boundary the use of concrete demolition
waste as replacement for primary
Type of EPD: cradle to gate with options, modules materials
C1–C4, and module D (A1–A3 + C + D and additional
modules A4, A5 and B1)
3.3 Estimates and assumptions
The selected system boundaries include the No estimates or assumptions were made that would be
production of the concrete including the extraction of relevant for the interpretation of the life cycle
raw materials through to the installation, use and end assessment results.
of life of the finished product.
3.4 Cut-off criteria
Material production and placement All raw materials for the production of concrete, all
transport as well as all energy and water consumption
Module A1: Extraction and for production, mixing, placing and waste treatment of
processing of the raw materials the concrete were taken into account.
used in concrete production
The environmental impacts from the production and
Module A2: Transport of the raw use of the formwork were neglected for the life cycle
materials to the plant assessment of the concrete production. With the usual
frequency of use of formwork, the mass of resources
Module A3: Concrete production in and primary energy used is less than 1% of the total
the plant and waste treatment values for concrete production. The materials used for
concrete curing were also excluded as they represent
less than 1% of the total mass and primary energy use
Module A4: Transport to the for concrete production.
construction site
3.5 Background data
Module A5: Includes all The CarbonCLARITYTM EN 15804 EPD Generator -
processes associated with placing RMX version 1.0.1 dated 27/05/2024 with configuration
the concrete (e.g. pumping or file dated 07/02/2025 was used for the life cycle
installation by crane) as well as the assessment.
production, transport and treatment
of unused concrete (e.g. return Datasets from EPDs and from the Ecoinvent database
concrete) (version 3.8) were used for the calculation.
Use phase 3.6 Data quality
The data basis for this EPD is the continuous data
Module B1: Carbonation during the acquisition in the RMX Timisoara 1 plant. The data
use phase collected were reviewed for plausibility by Climate
Earth and were rated as very good quality.
Module B2-B7: For concrete
components, maintenance, repair The background datasets are on average less than 5
refurbishment or replacement years old and their quality is overall rated as good or
measures are not usually required very good.
during the reference service life.
Therefore, no environmental
burden is considered in these
modules.
5 Environmental Product Declaration Holcim (Romania) SA – 833290 concrete, Plant RMX Timisoara 1
3.7 Period under review the combustion of combustible waste was only applied
For the life cycle assessment of the ECOPact to CO2 emissions, as other emissions (eg, NOx, SOx,
C20/25Cl02D16S3, data from the period 01/01/2023 to etc.) were not easily differentiated from the different
31/12/2023 were used. types of fuels.
3.8 Geographic Representativeness Energy and auxiliary materials used in the production
Land or region, in which the declared product system of concrete are allocated to each individual concrete
is manufactured, used or handled at the end of the mix based on the total volume of concrete produced in
product´s lifespan: Romania the plant.
3.9 Allocation Finally, the use of recycled and/or secondary raw
Cementitious products such as fly ash, blast furnace materials is allocated to each individual concrete mix
slag or silica fume are considered co-products and based on their actual composition.
economic allocation is used.
3.10 Comparability
The alternative fuels used for the production of the Basically, a comparison or an evaluation of EPD data
cements used are classified either as secondary fuels is only possible if all the data sets to be compared
or as waste. Emissions from secondary fuels are were created according to EN 15804 and the building
included in the impact assessment results while context, respectively the product-specific
emissions from waste fuels are reported as additional characteristics of performance, are taken into account.
information according to the IBU Cement PCR. The
waste status of the fuels concerned was verified using The Ecoinvent background database is used (version
their waste codes. The exclusion of the impact due to 3.8).
6 Environmental Product Declaration Holcim (Romania) SA – 833290 concrete, Plant RMX Timisoara 1
4. LCA: Scenarios and additional technical information
Information on describing the biogenic Carbon k∗√t
Content at factory gate CO uptake= ∗A∗D ∗C
2 1000 i c factor
Name Value Unit
Biogenic Carbon Content in
0 kg C
product where
Biogenic Carbon Content in
0 kg C
accompanying packaging k = k-factor sourced from EN 16757 standard
depending on structure type, exposure condition
Note: 1 kg biogenic Carbon is equivalent to 44/12 kg and concrete strength class [mm/year0,5]
of CO t = service life (yr)
2
A = area of concrete element (m2/m3)
i
Module A3: Manufacturing D c = degree of carbonation sourced from EN 16757
The carbon intensity of the electricity used in standard depending on structure type and exposure
manufacturing is 0.30 kgCO2eq./kWh. condition (%)
C = 106 (kg CO/m3). It is calculated as per EN
factor 2
Module A4: Transport to jobsite 16757 standard based on the concrete
The following table shows the data used in the composition
modelling of product transport to the jobsite:
Module B2-B7:
Transport to the building site (A4) No maintenance or repair is usually required for
Name Value Unit concrete during its reference service life. In addition,
lt diesel no energy or water are consumed during its use.
Litres of fuel (per m3 concrete) 4.50 eq./100
km* Module C1-C4:
Transport distance 9.43 km According to the current state of the art, structures
made of concrete and reinforced concrete are mainly
Capacity utilization (including
41.0 % dismantled with long-front excavators equipped with
empty runs)
demolition claws.
Gross density of products
2314.74 kg/m3
transported
Name Value Unit
Capacity utilization volume
0.82 - Diesel consumption for 2.9 lt/m3
factor
demolition process
* If trucks are not powered by diesel, the necessary energy
Demolition waste collected 2314.74 kg
consumption is converted into the equivalent diesel
consumption. Therefore the total fuel consumption can be
expressed in a single unit of liters of diesel equivalent / 100 In Romania 87% of concrete waste is recycled or used
km. for backfilling while 13% ends up in landfills (Eurostat).
Module A5: Installation of concrete Therefore, two scenarios for 100% recycling (Scenario
The following table shows the data used in the 1) and 100% landfill (Scenario 2) are considered in this
modelling of product installation: life cycle assessment.
Installation into the building (A5) After demolition the concrete debris is transported to
Name Value Unit the crushing plant (Scenario 1; C2/1) or landfill
Electricity consumption 0.26 kWh (Scenario 2;C2/2) according to the following details.
Other energy carriers 12.0 MJ
Material loss 6.26 kg Name Scenario 1 Scenario 2 Unit
Truck 29 29 km
Module B1: Carbonation
Through carbonation, concrete components absorb In Scenario 1 (100% recycling) the processing of
carbon dioxide from the air during their useful life. This concrete rubble is usually carried out using jaw or
can be expressed as a negative global warming impact crushers, which, in addition to pure breaking,
potential in module B1 and is calculated according to also perform a pre-screening and metal separation
EN 16757 using the following data. (C3/1). No impacts for waste disposal are reported
(C4/1).
Carbonation during use
Name Value Unit In Scenario 2 (100% landfill) the concrete debris
Structure type Building - without any further processing is landfilled (C4/2). No
Building, impacts for waste processing are reported (C3/2).
Exposure condition interior, with -
cover Name Scenario 1 Scenario 2 Unit
Service life 50 yr For reuse 0 0 kg
Area to volume ratio 5 m2/m3 For recycling 2314.74 0 kg
Weight per unit area 463 kg/m2 For landfill 0 2314.74 kg
Carbonation results for alternative scenarios can be The carbonation of concrete rubble during the end of
calculated using the following formula life phase is modelled according to the guidelines of
7 Environmental Product Declaration Holcim (Romania) SA – 833290 concrete, Plant RMX Timisoara 1
EN 16757 standard for both Scenario 1 (C3/1) and can be used for the production of new steel products.
Scenario 2 (C4/2). The results for Scenario 1 are reported in module D/1.
Module D: Benefits and loads beyond the system No Module D results (D/2) are calculated for Scenario
boundary 2 (100% landfill).
In Scenario 1 (100% recycling), the output at the end
of the crushing process can replace the primary The benefits in the LCA results for the replacement of
materials sand / gravel and crushed stone as primary raw materials are shown in module D.
secondary material. Potentially recovered steel fibers
8 Environmental Product Declaration Holcim (Romania) SA – 833290 concrete, Plant RMX Timisoara 1
5. LCA: Results
The table below contains the life cycle assessment results for a declared unit of 1 m3 of unreinforced concrete
ECOPact C20/25Cl02D16S3.
The characterization factors of the "Environmental Footprint reference Package 3.0" were used to determine the
LCA results.
DESCRIPTION OF THE SYSTEM BOUNDARY (X = INCLUDED IN LCA; ND = MODULE OR INDICATOR NOT
DECLARED; MNR = MODULE NOT RELEVANT)
BENEFITS AND
CONSTRUCTI LOADS
PRODUCT STAGE ON PROCESS USE STAGE END OF LIFE STAGE BEYOND THE
STAGE SYSTEM
BOUNDARIES
ylppus
lairetam
waR
tropsnarT
gnirutcafunaM
etag
eht
morf
tropsnarT
etis
eht
ot
ylbmessA
esU
ecnanetniaM
riapeR
tnemecalpeR tnemhsibrufeR
esu
ygrene
lanoitarepO
esu
retaw
lanoitarepO
noitcurtsnoc-eD
noitilomed tropsnarT
gnissecorp
etsaW
lasopsiD -esueR -yrevoceR -gnilcyceR laitnetop
A1 A2 A3 A4 A5 B1 B2 B3 B4 B5 B6 B7 C1 C2 C3 C4 D
x x x x x x ND MNR MNR MNR ND ND x x x x x
RESULTS OF THE LCA - ENVIRONMENTAL IMPACT according to EN 15804+A2: 1 m³ ECOPact
C20/25Cl02D16S3
Core
Unit A1-A3 A4 A5 B1 C1 C2/1 C2/2 C3/1 C3/2 C4/1 C4/2 D/1 D/2
Indicator
GWP-total [kg CO2-Eq.] 168 3.21 1.62 -10.4 9.53 6.23 6.23 -0.20 0 0 8.24 -8.23 0
GWP-fossil [kg CO2-Eq.] 168 3.21 1.62 -10.4 9.53 6.23 6.23 -0.20 0 0 8.22 -8.20 0
GWP-biogenic [kg CO2-Eq.] 0.19 1.4E-3 6.49E-4 0 1.25E-3 1.7E-3 1.7E-3 9.26E-4 0 0 5.45E-3 -0.03 0
GWP-luluc [kg CO2-Eq.] 0.02 1.41E-3 1.25E-4 0 1.01E-3 2.42E-3 2.42E-3 3.4E-4 0 0 0.01 -4.84E-3 0
ODP [kg CFC11-Eq.] 1.1E-5 7.43E-7 2.74E-7 0 2.06E-6 1.42E-6 1.42E-6 5.04E-7 0 0 4.93E-6 -8.5E-7 0
AP [mol H+-Eq.] 0.40 9.39E-3 0.01 0 0.10 0.03 0.03 0.03 0 0 0.11 -0.08 0
EP-freshwater [kg P-Eq.] 7.84E-3 2.29E-46.41E-5 0 2.98E-4 4.56E-4 4.56E-4 5.79E-4 0 0 1.12E-3-2.05E-3 0
EP-marine [kg N-Eq.] 0.14 1.93E-3 5.58E-3 0 0.04 7.98E-3 7.98E-3 0.01 0 0 0.04 -0.02 0
EP-terrestrial [mol N-Eq.] 1.55 0.02 0.06 0 0.49 0.09 0.09 0.11 0 0 0.44 -0.23 0
POCP [kg NMVOC-Eq.] 0.39 5.43E-3 0.02 0 0.13 0.03 0.03 0.03 0 0 0.13 -0.05 0
ADPE [kg Sb-Eq.] 1.26E-4 1.26E-5 9.12E-7 0 5.08E-6 1.48E-5 1.48E-5 6.71E-6 0 0 2.82E-5-1.32E-4 0
ADPF [MJ] 953 49.0 19.4 0 132 96.3 96.3 63.8 0 0 340 -111 0
WDP [m³ world-Eq depr.] 33.3 0.16 0.13 0 0.21 0.37 0.37 0.56 0 0 15.3 25.1 0
GWP = Global warming potential; ODP = Depletion potential of the stratospheric ozone layer; AP = Acidification potential of land and
water; EP = Eutrophication potential; POCP = Formation potential of tropospheric ozone photochemical oxidants; ADPE = Abiotic
Legend
depletion potential for non fossil resources; ADPF = Abiotic depletion potential for fossil resources; WDP = Water (user) deprivation
potential
RESULTS OF THE LCA - INDICATORS TO DESCRIBE RESOURCE USE according to EN 15804+A2: 1 m3
ECOPact C20/25Cl02D16S3
Indicator Unit A1-A3 A4 A5 B1 C1 C2/1 C2/2 C3/1 C3/2 C4/1 C4/2 D/1 D/2
PERE [MJ] 180 0.76 0.95 0 0.74 1.07 1.07 8.79 0 0 2.90 -24.4 0
PERM [MJ] 27.5 0 0.07 0 0 0 0 0 0 0 0 0 0
PERT [MJ] 207 0.76 1.03 0 0.74 1.07 1.07 8.79 0 0 2.90 -24.4 0
PENRE [MJ] 934 49.0 19.4 0 132 96.3 96.3 63.8 0 0 341 -111 0
PENRM [MJ] 18.6 0 0.05 0 0 0 0 0 0 0 0 0 0
PENRT [MJ] 953 49.0 19.4 0 132 96.3 96.3 63.8 0 0 341 -111 0
SM [kg] 2.67 0 7.21E-3 0 0 0 0 0 0 0 0 2312 0
RSF [MJ] 137 0 0.37 0 0 0 0 0 0 0 0 0 0
NRSF [MJ] 164 0 0.44 0 0 0 0 0 0 0 0 0 0
FW [m³] 3.31 7.59E-3 0.01 0 6.47E-3 0.01 0.01 0.05 0 0 0.36 -1.81 0
PERE = Use of renewable primary energy excluding renewable primary energy resources used as raw materials; PERM = Use of
renewable primary energy resources used as raw materials; PERT = Total use of renewable primary energy resources; PENRE
= Use of non-renewable primary energy excluding nonrenewable primary energy resources used as raw materials; PENRM =
Legend
Use of non-renewable primary energy resources used as raw materials; PENRT = Total use of non-renewable primary energy
resources; SM = Use of secondary material; RSF = Use of renewable secondary fuels; NRSF = Use of non-renewable secondary
fuels; FW = Use of net freshwater
9 Environmental Product Declaration Holcim (Romania) SA – 833290 concrete, Plant RMX Timisoara 1
RESULTS OF THE LCA – WASTE CATEGORIES AND OUTPUT FLOWS according to EN 15804+A2: 1 m3
ECOPact C20/25Cl02D16S3
Indicator Unit A1-A3 A4 A5 B1 C1 C2/1 C2/2 C3/1 C3/2 C4/1 C4/2 D/1 D/2
HWD [kg] 0.84 0.04 0.01 0 0.10 0.09 0.09 0.14 0 0 0.23 -0.75 0
NHWD [kg] 38.3 3.13 0.20 0 0.55 9.50 9.50 1.20 0 0 2316 -7.61 0
RWD [kg] 7.96E-3 3.3E-4 1.52E-4 0 9.12E-4 6.37E-4 6.37E-4 7.01E-4 0 0 2.23E-3-1.35E-3 0
CRU [kg] 0 0 0 0 0 0 0 0 0 0 0 0 0
MFR [kg] 2.78E-3 0 7.53E-6 0 0 0 0 2315 0 0 0 0 0
MER [kg] 0 0 0 0 0 0 0 0 0 0 0 0 0
EEE [MJ] 0 0 0 0 0 0 0 0 0 0 0 0 0
EET [MJ] 0 0 0 0 0 0 0 0 0 0 0 0 0
HWD = Hazardous waste disposed; NHWD = Nonhazardous waste disposed; RWD = Radioactive waste disposed; CRU =
Legend Components for reuse; MFR = Materials for recycling; MER = Materials for energy recovery; EEE = Exported electrical energy;
EEE = Exported thermal energy
RESULTS OF THE LCA – additional impact categories according to EN 15804+A2: 1 m3 ECOPact
C20/25Cl02D16S3
Indicator Unit A1-A3 A4 A5 B1 C1 C2/1 C2/2 C3/1 C3/2 C4/1 C4/2 D/1 D/2
[Disease
PM 4.27E-62.21E-7 3.21E-7 0 2.68E-6 7.25E-7 7.25E-7 5.46E-7 0 0 2.31E-6-1.06E-6 0
Incidence]
IRP [kBq U235-Eq.] 9.77 0.26 0.17 0 0.60 0.45 0.45 1.74 0 0 1.51 -3.09 0
ETP-fw [CTUe] 508 39.7 6.97 0 36.7 32.6 32.6 33.0 0 0 93.7 -158 0
2.87E-
HTP-c [CTUh] 3.4E-8 1.33E-9 0 2.99E-9 2.1E-9 2.1E-9 9.7E-10 0 0 5.45E-9-1.23E-8 0
10
HTP-nc [CTUh] 1.45E-64.15E-8 1.01E-8 0 5.61E-8 8.32E-8 8.32E-8 2.06E-8 0 0 1.41E-7-2.03E-7 0
SQP [-] 1223 54.7 4.68 0 16.8 109 109 9.54 0 0 715 -282 0
PM = Potential incidence of disease due to PM emissions; IRP = Potential Human exposure efficiency relative to U235;
Legend ETPfw = Potential comparative Toxic Unit for ecosystems; HTPc = Potential comparative Toxic Unit for humans (cancerogenic);
HTPnc = Potential comparative Toxic Unit for humans (not cancerogenic); SQP = Potential soil quality index
nuclear fuel cycle. It does not consider effects due
On Global Warming Potential (GWP): to possible nuclear accidents, occupational
Net values are declared for all GWP indicators in A1 exposure nor radioactive waste disposal in
– A3. The waste status of the (waste-based) fuels underground facilities. Potential ionizing radiation
used in cement production has been verified. Gross from the soil, radon and from some construction
emissions (i.e. including CO from incineration of materials is also not measured by this indicator.
2
waste) are 184 kg CO-eq. / t (GWP-total), 183 kg
2
CO-eq. / t (GWP fossil), 0.19 kg CO eq. / t (GWP-
2 2 Disclaimer 2 –for the indicators: “abiotic depletion
biogenic).
potential for fossil resources”, “abiotic depletion
potential for non-fossil resources”, “water (user)
For wastes with biogenic carbon content, gross CO deprivation potential”, “deprivation-weighted water
2
emissions correspond to the uptake of biogenic consumption”, “potential comparative toxic unit for
CO2 during the biomass growth phase. ecosystems”, “potential comparative toxic unit for
humans - cancer effects”, “potential comparative
toxic unit for humans – non-cancer effects”,
Disclaimer 1 – for the indicator “potential Human
“potential soil quality index”. The results of this
exposure efficiency relative to U235“. This impact
environmental impact indicator shall be used with
category deals mainly with the eventual impact of
care as the uncertainties on these results are high
low dose ionizing radiation on human health of the
or as there is limited experience with the indicator.
10 Environmental Product Declaration Holcim (Romania) SA – 833290 concrete, Plant RMX Timisoara 1
6. LCA: Interpretation
The following table shows the most important influencing factors on important indicators of the impact and life
cycle inventory analysis.
Category GWP AP EP POCP PERT PENRT ADPE FW PM
total terrestrial
Cement 84.9 % 68.9 % 73.4 % 70.0 % 90.2 % 57.7 % 17.2 % 7.21 % 35.8 %
Aggregate 3.30 % 11.8 % 10.7 % 10.3 % 4.56 % 8.82 % 49.9 % 78.7 % 19.2 %
Cementitious 0 % 0 % 0 % 0 % 0 % 0 % 0 % 0 % 0 %
Fibers 0 % 0 % 0 % 0 % 0 % 0 % 0 % 0 % 0 %
Admixtures 1.59 % 0.87 % 0.67 % 0.73 % 1.85 % 5.20 % 0.21 % 0.29 % 0.88 %
Other materials
and processes 10.2 % 18.4 % 15.1 % 19.0 % 3.38 % 28.3 % 32.7 % 13.8 % 44.1 %
Total 100% 100% 100% 100% 100% 100% 100% 100% 100%
Cement: Includes the impacts for the production of all cements used. Aggregate: Includes the impacts for the production
of sand and gravel. Cementitious: Includes the impacts for the production of all cementitious materials used such as
Legend slag, fly ash or limestone. Fibers: Includes the impacts for the production of fibers. Admixtures: Includes the impacts for
the production of concrete admixtures such as plasticisers or retarders. Other materials and processes: Includes the
impacts of materials or production processes not covered by the above categories.
In the production of concrete, cement production materials. The contribution of other processes in the
dominates all impact categories. This applies in plant is low, especially with regard to greenhouse,
particular to the global warming potential (GWP). acidification and eutrophication impact categories.
Another major influencing factor is the
extraction/production and transport of the raw
7. Requisite evidence
7.1 Radioactivity concentrations will equate to an annual effective dose
Measurements of the specific activity (gamma of about 0.25 mSv (excess to the dose received
spectrometry) in Europe resulted in the following outdoors) (Radiation Protection 112).
typical values for concrete (Radiation Protection 112)
(in Bq/kg concrete). In Romania there are currently no statutory limit values
for assessing the radioactivity of building materials.
Element Typical values (max values)
7.2 VOC emissions and leaching
RA226 40 (240)
The environmental compatibility of concrete is ensured
Th228 30 (190)
by the fact that only standardized starting materials
K40 400 (1600)
may be used that are a priori regarded as harmless.
Therefore, no tests are normally carried out for VOC
Radiation exposure in an apartment block made of emissions and leaching of concrete.
concrete with the above average activity
8. References
Standards EN 1992-1-2:2004+A1:2019, Eurocode 2. Design of
concrete structures - General rules. Structural fire
EN 12350 design
EN 12350-4:2019 Testing fresh concrete
EN ISO 14025
EN 12390 EN ISO 14025:2011, Environmental labels and
declarations. Type III environmental declarations.
EN 12390-3:2019 Testing hardened concrete
Principles and procedures
EN 13501-1
EN 15804
EN 13501-1:2018, Fire classification of construction
EN 15804:2012+A2+AC:2021, Sustainability of
products and building elements - Classification using
construction works. Environmental product
data from reaction to fire tests
declarations. Core rules for the product category of
construction products
EN 13501-2
EN 13501-2:2016 Fire classification of construction
EN 16757
products and building elements. Classification using
EN 16757:2022. Sustainability of construction works.
data from fire resistance tests, excluding ventilation
Environmental product declarations. Product Category
services
Rules for concrete and concrete elements
EN 1992-1-2
11 Environmental Product Declaration Holcim (Romania) SA – 833290 concrete, Plant RMX Timisoara 1
EN-206-1
EN 206:2013+A2:2021, Concrete - Specification, PCR Part B
performance, production and conformity Product category rules on Guidance-Texts for Building-
Related Products and Services. Part B: Requirements
Other literature on the EPD for Concrete components made of in-situ
or ready-mixed concrete, V6, Berlin: Institut Bauen und
CarbonCLARITYTM EN 15804 EPD Generator - RMX Umwelt e.V. 17/07/2023
Version 1.0.1 dated 27/05/2024
www.climateearth.com
ECHA
European Chemicals Agency (ECHA): Candidate List
of Substances of Very High Concern for Authorization.
https://echa.europa.eu/
Eurostat
Statistical Office of the European Union
https://ec.europa.eu/eurostat/databrowser/view/env_w
astrt/default/table?lang=en
Ecoinvent
Database, version 3.8, Ecoinvent, 2021.
EF 3.0
Environmental Footprint, ref package 3.0, November
2019 (European Platform on Life Cycle Assessment
(EPLCA))
IBU 2021
Institut Bauen und Umwelt e.V.: General instructions
for the EPD program of Institut Bauen und Umwelt e.V.
Version 2.0, Berlin: Institut Bauen und Umwelt e.V.,
2021. www.ibu-epd.com
No 528/2012
Regulation (EU) No 528/2012 of the European
Parliament and of the Council of 22 May 2012
concerning the making available on the market and
use of biocidal products
Radiation Protection 112
European Commission, Directorate-General for
Environment, Radiological protection principles
concerning the natural radioactivity of building
materials, Publications Office, 2000
REACH Regulation
Registration, Evaluation, Authorisation and Restriction
of Chemicals, EG 1907/2006:2006-12-18
WCO
Waste Catalog Ordinance (WCO), December 10th
2001
PCR Part A
Product category rules for building related products
and services. Part A: Calculation rules for the life cycle
assessment and requirements for the project report
according to EN 15804+A2:2021 (v1.3). Berlin: Institut
Bauen und Umwelt e.V., 31/08/2022
PCR Cement
Product category rules for building related products
and services. Part B: Requirements for the EPD for
cement, version 5. Berlin: Institut Bauen und Umwelt
e.V. (ed.), 04/07/2023. www.ibu-epd.com
12 Environmental Product Declaration Holcim (Romania) SA – 833290 concrete, Plant RMX Timisoara 1
Publisher
IBU - Institut Bauen und Umwelt e.V. Tel +49 (0)30 3087748 - 0
Hegelplatz 1 Fax +49 (0)30 3087748 - 29
10117 Berlin Mail info@ibu-epd.com
Germany Web www.ibu-epd.com
Programme holder
IBU - Institut Bauen und Umwelt e.V. Tel +49 (0)30 3087748 - 0
Hegelplatz 1 Fax +49 (0)30 3087748 - 29
10117 Berlin Mail info@ibu-epd.com
Germany Web www.ibu-epd.com
Author of the Life Cycle
Assessment
Climate Earth, Inc. Tel +1 (415) 391-2725
137 Park Place, Suite 204 Mail info@climateearth.com
Point Richmond, CA 94801 Web www.climateearth.com
United States
Owner of the Declaration
Holcim (Romania) SA Tel
46D-46E-48, Pipera Road, Oregon Mail simona.stefan@holcim.com
Park - Building B, 6th Floor Web holcim.ro
020309 Bucharest
Romania
13 Environmental Product Declaration Holcim (Romania) SA – 833290 concrete, Plant RMX Timisoara 1
