ENVIRONMENTAL PRODUCT DECLARATION
as per ISO 14025 and EN 15804+A2
Owner of the Declaration Aggregate Industries
Programme holder Institut Bauen und Umwelt e.V. (IBU)
Publisher Institut Bauen und Umwelt e.V. (IBU)
Declaration number IBU-CEI-HOL-2205120-UK2024001520-ISUE002-EN
Issue date 05/08/2024
Valid to 04/08/2029
Concrete C32/40 CIIIA WTT ECOPact produced in plant
Hornsey
Mix code HNL2930/009, EPD Version 2
Aggregate Industries
www.ibu-epd.com | https://epd-online.com
1. General Information
Aggregate Industries C32/40 CIIIA WTT ECOPact
Programme holder Owner of the declaration
IBU - Institut Bauen und Umwelt e.V. Aggregate Industries
Hegelplatz 1 Bardon Hall
10117 Berlin LE67 1TL Coalville
Germany United Kingdom
Declaration number Declared product / Declared unit
IBU-CEI-HOL-2205120-UK2024001520-ISUE002-EN 1 m3 of unreinforced concrete C32/40 CIIIA
WTT ECOPact
This declaration is based on the product Scope:
category rules: This document refers to the production of
Concrete components made of in-situ or ready- C32/40 CIIIA WTT ECOPact concrete, mix
mixed concrete, 03.2022 (PCR checked and code HNL2930/009 produced in the plant of
approved by the SVR) Hornsey of Aggregate Industries in United
Kingdom for use as concrete in building
Issue date construction and civil engineering.
05/08/2024
The EPD was calculated with the pre-verified
Valid to software CarbonCLARITYTM EN 15804 EPD
04/08/2029 Generator - RMX of Climate Earth.
The owner of the declaration shall be liable for
the underlying information and evidence; the
IBU shall not be liable with respect to
manufacturer information, life cycle assessment
data and evidences.
The EPD was created according to the
specifications of EN 15804+A2. In the following,
the standard is simply referred to as EN 15804.
Verification
The standard EN 15804 serves as the core PCR
Independent verification of the declaration and data
according to ISO 14025:2011
Hans Peters internally x externally
(Chairman Institut Bauen und Umwelt e.V.)
Florian Pronold Matthias Schulz
(Managing Director Institut Bauen und Umwelt e.V.) (Independent verifier)
2 Environmental Product Declaration Aggregate Industries – HNL2930/009 concrete, Plant Hornsey
2. Product
2.1 Product description/Product definition 2.4 Delivery status
Concrete is produced by mixing cement, aggregates Fresh concrete is delivered to the customers in
and water with potentially additional cementitious concrete truck mixers. It can also be picked up by the
materials, fibers and additives. client using their trucks.
The fresh concrete is generally poured into formwork, 2.5 Base materials/Ancillary materials
compacted and hardened in the desired form by Name Value Unit
hydration of the cement to form a solid artificial rock. Cement ca. 10-17 M.%
Water ca. 7-10 M.%
The declared product is unreinforced concrete that is Aggregate ca. 70-90 M.%
delivered to the job site as ready-mix concrete. In the
Cementitious ca. 7-10 M.%
case of reinforced components, the proportion of
Fibers ca. <1 M.%
reinforcing steel must be taken into account
separately. Admixtures ca. <1 M.%
Water resisting admixtures are added to improve the
impermeability of concrete and render it waterproof.
To calculate the life cycle assessment of the C32/40
CIIIA WTT ECOPact concrete in plant Hornsey, the
production data from mix code HNL2930/009 were
used.
For the use and application of the product the
respective national provisions at the place of use
apply, such as the building codes and the
corresponding national specifications.
Note: dashed lines indicate production steps that do not
2.2 Application
necessarily apply to this concrete
Concrete is a widely used building material in the
construction industry. It is used for example for the This product contains substances listed in the ECHA
construction of walls, stairs, floor, foundations, bored candidate list (date: 14.06.2023) exceeding 0.1
piles or even complete structures such as bridges. percentage by mass: no
2.3 Technical data This product contains other CMR substances in
Concrete C32/40 CIIIA WTT ECOPact has the categories 1A or 1B which are not on the candidate
following technical properties: list, exceeding 0.1 percentage by mass: no
Technical data Biocide products were added to this construction
Name Value Unit product or it has been treated with biocide products
Gross density 2380 kg/m3 (this then concerns a treated product as defined by the
Compressive (EU) Ordinance on Biocide Products No. 528/2012): no
C32/40 N/mm2
strength
2.6 Manufacture
The dosed aggregates are first premixed with cement
This concrete product is produced according to
as a binding agent and other additives. The mixture is
standard BS 8500:2023 Concrete - Complementary
then mixed with water to form a plastically deformable
British Standard to BS EN 206 as a designed concrete.
fresh concrete. This is transported to the customer
where it is placed in the prepared formwork and
This technical data fulfill the requirements according to
compacted.
BS 8500 standard regarding quality control and
conformity checks. Testing is done according to EN
To ensure the quality of the concrete, quality
12350 and EN 12390. Further technical data, as
assurance systems is installed in Hornsey plant, which
indicated in PCR B, are not relevant for this product.
is based on the requirements for in-house production
This is because properties such as thermal
control in BS 8500 standard.
conductivity, tensile strength or modulus of elasticity
can be found in the regulations for the design of
2.7 Environment and health during manufacturing
concrete components and are therefore not routinely
Fresh concrete and residual water recycling is
checked.
common practice in the Hornsey plant. Not yet
hardened concrete residues from mixers, concrete
Performance characteristics for fresh concrete in
vehicles, bucket conveyors and concrete distributors
relation to its characteristics according to the relevant
are washed out and both the aggregate and the
technical regulation (no CE marking).
remaining water are reused as concrete raw materials.
3 Environmental Product Declaration Aggregate Industries – HNL2930/009 concrete, Plant Hornsey
Fresh concrete contains a strongly alkaline solution Fire
that is created when cement is mixed with water and According to EN 13501-1, concrete meets the
can cause skin and eye irritation. The abrasiveness of requirements of building material class A1, "non-
the aggregate used can also support this irritation. flammable". In the event of fire, no toxic gases and
vapors can arise, and burning concrete components do
Cements used within this product are low in chromate, not drip or fall off.
as per requirements of REACH regulation, in order to
limit the development of allergic chromate dermatitis High fire resistance classes can be achieved through
that can happen in the event of prolonged contact with appropriate dimensioning of the components (in EN
the concrete. 1992-1-2 tabular values for fire resistance classes
according to EN 13501-2 are given).
Further information can be found in the safety data
sheets. Fire protection
https://www.aggregate.com/news-and-resources/ Name Value
technical-information/safety-data-sheets Building material class A1 "not combustible"
2.8 Product processing/Installation
Water
In general, after mixing the concrete is transported to
When exposed to water (e.g. floods), concrete is
the construction site with trucks, placed in the prepared
largely inert. No substances are washed out in
formwork by direct pouring or pumping and usually
quantities that could be hazardous to water.
compacted with internal vibrators. After a sufficiently
long hardening time, the formwork is removed and the
concrete is cured further with time. Mechanical destruction
The mechanical destruction of concrete, e.g. by
demolishing concrete, does not produce any
2.9 Packaging
substances that are hazardous to the environment or
The delivery of concrete does not require the use of
health.
packaging material.
2.14 Re-use phase
2.10 Condition of use
Components made of concrete can be dismantled. The
The composition of the concrete does not
concrete is first crushed and separated into individual
fundamentally change when it is used.
grain fractions and used in road construction or in
small proportions as recycled aggregate for the
2.11 Environment and health during use
production of fresh concrete. If steel fibers or rebar is
The natural ionizing radiation from concrete is low and
included in the concrete, this is separated during or
harmless to health. The environmental compatibility of
after demolition and reused as scrap. Recovery of
concrete is ensured by the fact that only standardized
alternative fibers or rebar is not commonplace.
starting materials may be used that are a priori
regarded as harmless.
2.15 Disposal
For construction waste made of concrete, the waste
2.12 Reference service life
codes 17 01 01 (concrete), 17 04 05 (steel fibers) and
A reference service of 50 years is used for modeling
17 02 13 (plastic fibers) (WCO) apply in accordance
concrete’s use phase.
with the European list of waste.
2.13 Extraordinary effects
2.16 Further information
Further information www.aggregate.com.
4 Environmental Product Declaration Aggregate Industries – HNL2930/009 concrete, Plant Hornsey
3. LCA: Calculation rules
3.1 Declared unit
1 m3 of unreinforced concrete C32/40 CIIIA WTT
ECOPact End of life
In the case of reinforced components, the proportion of Module C1: Dismantling /
reinforcing steel must be taken into account demolition of concrete buildings /
separately. components
Declared unit Module C2: Transport of
Designation Value unit demolished concrete for processing
Declared unit 1 m3
Module C3: Concrete waste
Density 2380 kg/m3
processing
Conversion factor to 1 kg 4.2E-4 -
Module C4: Concrete waste
To calculate the life cycle assessment of the C32/40 disposal
CIIIA WTT ECOPact concrete in plant Hornsey, the
production data from mix code HNL2930/009 were Module D
used.
Module D: Benefits and loads for
3.2 System boundary the use of concrete demolition
waste as replacement for primary
Type of EPD: cradle to gate with options, modules materials
C1–C4, and module D (A1–A3 + C + D and additional
modules A4, A5 and B1)
3.3 Estimates and assumptions
The selected system boundaries include the No estimates or assumptions were made that would be
production of the concrete including the extraction of relevant for the interpretation of the life cycle
raw materials through to the installation, use and end assessment results.
of life of the finished product.
3.4 Cut-off criteria
Material production and placement All raw materials for the production of concrete, all
transport as well as all energy and water consumption
Module A1: Extraction and for production, mixing, placing and waste treatment of
processing of the raw materials the concrete were taken into account.
used in concrete production
The environmental impacts from the production and
Module A2: Transport of the raw use of the formwork were neglected for the life cycle
materials to the plant assessment of the concrete production. With the usual
frequency of use of formwork, the mass of resources
Module A3: Concrete production in and primary energy used is less than 1% of the total
the plant and waste treatment values for concrete production. The materials used for
concrete curing were also excluded as they represent
less than 1% of the total mass and primary energy use
Module A4: Transport to the for concrete production.
construction site
3.5 Background data
Module A5: Includes all The CarbonCLARITYTM EN 15804 EPD Generator -
processes associated with placing RMX version 1.0.1 dated 27/05/2024 with configuration
the concrete (e.g. pumping or file dated 19/10/2023 was used for the life cycle
installation by crane) as well as the assessment.
production, transport and treatment
of unused concrete (e.g. return Datasets from EPDs and from the Ecoinvent database
concrete) (version 3.8) were used for the calculation.
Use phase 3.6 Data quality
The data basis for this EPD is the continuous data
Module B1: Carbonation during the acquisition in the Hornsey plant. The data collected
use phase were reviewed for plausibility by Climate Earth and
were rated as very good quality.
Module B2-B7: For concrete
components, maintenance, repair The background datasets are on average less than 5
refurbishment or replacement years old and their quality is overall rated as good or
measures are not usually required very good.
during the reference service life.
Therefore, no environmental
burden is considered in these
modules.
5 Environmental Product Declaration Aggregate Industries – HNL2930/009 concrete, Plant Hornsey
3.7 Period under review the combustion of combustible waste was only applied
For the life cycle assessment of the C32/40 CIIIA WTT to CO2 emissions, as other emissions (eg, NOx, SOx,
ECOPact, data from the period 01/07/2021 to etc.) were not easily differentiated from the different
30/06/2022 were used. types of fuels.
3.8 Geographic Representativeness Energy and auxiliary materials used in the production
Land or region, in which the declared product system of concrete are allocated to each individual concrete
is manufactured, used or handled at the end of the mix based on the total volume of concrete produced in
product´s lifespan: United Kingdom the plant.
3.9 Allocation Finally, the use of recycled and/or secondary raw
Cementitious products such as fly ash, blast furnace materials is allocated to each individual concrete mix
slag or silica fume are considered co-products and based on their actual composition.
economic allocation is used.
3.10 Comparability
The alternative fuels used for the production of the Basically, a comparison or an evaluation of EPD data
cements used are classified either as secondary fuels is only possible if all the data sets to be compared
or as waste. Emissions from secondary fuels are were created according to EN 15804 and the building
included in the impact assessment results while context, respectively the product-specific
emissions from waste fuels are reported as additional characteristics of performance, are taken into account.
information according to the IBU Cement PCR. The
waste status of the fuels concerned was verified using The Ecoinvent background database is used (version
their waste codes. The exclusion of the impact due to 3.8).
6 Environmental Product Declaration Aggregate Industries – HNL2930/009 concrete, Plant Hornsey
4. LCA: Scenarios and additional technical information
Information on describing the biogenic Carbon where
Content at factory gate
Name Value Unit k = k-factor sourced from EN 16757 standard
Biogenic Carbon Content in depending on structure type, exposure condition
0 kg C
product and concrete strength class [mm/year0,5]
Biogenic Carbon Content in t = service life (yr)
0 kg C
accompanying packaging A = area of concrete element (m2/m3)
i
D = degree of carbonation sourced from EN 16757
c
Note: 1 kg biogenic Carbon is equivalent to 44/12 kg standard depending on structure type and exposure
of CO condition (%)
2
C = 149 (kg CO/m3). It is calculated as per EN
factor 2
Module A4: Transport to jobsite 16757 standard based on the concrete
The following table shows the data used in the composition
modelling of product transport to the jobsite:
Module B2-B7:
Transport to the building site (A4) No maintenance or repair is usually required for
Name Value Unit concrete during its reference service life. In addition,
lt diesel no energy or water are consumed during its use.
Litres of fuel (per m3 concrete) 4.60 eq./100
km* Module C1-C4:
Transport distance 3.14 km According to the current state of the art, structures
Capacity utilization (including made of concrete and reinforced concrete are mainly
45.6 %
empty runs) dismantled with long-front excavators equipped with
Gross density of products demolition claws.
2380 kg/m3
transported
Capacity utilization volume Name Value Unit
factor 0.91 - Diesel consumption for 2.9 lt/m3
demolition process
* If trucks are not powered by diesel, the necessary energy
consumption is converted into the equivalent diesel Demolition waste collected 2380 kg
consumption. Therefore the total fuel consumption can be
expressed in a single unit of liters of diesel equivalent / 100 In United Kingdom 97% of concrete waste is recycled
km. or used for backfilling while 3% ends up in landfills
(DEFRA).
Module A5: Installation of concrete
The following table shows the data used in the
Therefore, one scenario for 100% recycling is
modelling of product installation:
considered in this life cycle assessment.
Installation into the building (A5)
After demolition the concrete debris is transported to
Name Value Unit
the crushing plant according to the following details.
Electricity consumption 0.25 kWh
Other energy carriers 18.4 MJ
Name Value Unit
Material loss 47.2 kg Truck 25 km
Module B1: Carbonation The processing of concrete rubble is usually carried
Through carbonation, concrete components absorb out using jaw or impact crushers, which, in addition to
carbon dioxide from the air during their useful life. This pure breaking, also perform a pre-screening and metal
can be expressed as a negative global warming separation.
potential in module B1 and is calculated according to
EN 16757 using the following data. Name Value Unit
For reuse 0 kg
Carbonation during use For recycling 2380 kg
Name Value Unit For landfill 0 kg
Structure type Building -
Building,
The carbonation of concrete rubble during the end of
Exposure condition exterior, in -
life phase is modelled according to the guidelines of
ground
EN 16757 standard.
Service life 50 yr
Area to volume ratio 5 m2/m3 Module D: Benefits and loads beyond the system
Weight per unit area 476 kg/m2 boundary
The output at the end of the crushing process can
Carbonation results for alternative scenarios can be replace the primary materials sand / gravel and
calculated using the following formula crushed stone as secondary material. Potentially
recovered steel fibers can be used for the production
k∗√t of new steel products.
CO uptake= ∗A ∗D ∗C
2 1000 i c factor
The net output flow calculation in Module D considers
secondary material input flows from aggregates and
7 Environmental Product Declaration Aggregate Industries – HNL2930/009 concrete, Plant Hornsey
fibers while excluding small secondary material inputs
from other raw materials such as cement, cementitious The benefits in the LCA results for the replacement of
or admixtures. Additional output flows from the A5 life primary raw materials are shown in module D.
cycle stage are also excluded.
8 Environmental Product Declaration Aggregate Industries – HNL2930/009 concrete, Plant Hornsey
5. LCA: Results
The table below contains the life cycle assessment results for a declared unit of 1 m3 of unreinforced concrete
C32/40 CIIIA WTT ECOPact.
The characterization factors of the "Environmental Footprint reference Package 3.0" were used to determine the
LCA results.
DESCRIPTION OF THE SYSTEM BOUNDARY (X = INCLUDED IN LCA; ND = MODULE OR INDICATOR NOT
DECLARED; MNR = MODULE NOT RELEVANT)
BENEFITS AND
CONSTRUCTI LOADS
PRODUCT STAGE ON PROCESS USE STAGE END OF LIFE STAGE BEYOND THE
STAGE SYSTEM
BOUNDARIES
ylppus
lairetam
waR
tropsnarT
gnirutcafunaM
etag
eht
morf
tropsnarT
etis
eht
ot
ylbmessA esU
ecnanetniaM
riapeR
tnemecalpeR tnemhsibrufeR
esu
ygrene
lanoitarepO
esu
retaw
lanoitarepO
noitcurtsnoc-eD
noitilomed tropsnarT
gnissecorp
etsaW
lasopsiD -esueR -yrevoceR -gnilcyceR laitnetop
A1 A2 A3 A4 A5 B1 B2 B3 B4 B5 B6 B7 C1 C2 C3 C4 D
x x x x x x ND MNR MNR MNR ND ND x x x x x
RESULTS OF THE LCA - ENVIRONMENTAL IMPACT according to EN 15804+A2: 1 m³ C32/40 CIIIA WTT
ECOPact
Core
Unit A1-A3 A4 A5 B1 C1 C2 C3 C4 D
Indicator
GWP-total [kg CO2-Eq.] 251 0.91 6.87 -3.59 9.00 4.37 1.38 0 -4.20
GWP-fossil [kg CO2-Eq.] 250 0.91 6.86 -3.59 9.00 4.37 1.38 0 -4.19
GWP-biogenic [kg CO2-Eq.] 0.25 1.17E-4 5.1E-3 0 7.31E-4 3.42E-4 7.76E-4 0 -4.86E-3
GWP-luluc [kg CO2-Eq.] 0.02 1.39E-5 4.51E-4 0 2.22E-4 7.89E-5 1.66E-4 0 -2.75E-4
ODP [kg CFC11-Eq.] 6.16E-6 2.14E-7 5.23E-7 0 2.02E-6 9.67E-7 5.74E-7 0 -7.09E-7
AP [mol H+-Eq.] 0.82 2.25E-3 0.03 0 0.10 0.01 0.02 0 -0.03
EP-freshwater [kg P-Eq.] 9.27E-3 6.7E-6 2.72E-4 0 5.4E-5 8.08E-5 1.19E-3 0 -7.11E-4
EP-marine [kg N-Eq.] 0.21 7.14E-4 0.01 0 0.04 4.67E-3 0.01 0 -0.01
EP-terrestrial [mol N-Eq.] 2.38 5.55E-3 0.14 0 0.48 0.05 0.11 0 -0.15
POCP [kg NMVOC-Eq.] 0.62 1.11E-3 0.03 0 0.11 0.01 0.03 0 -0.04
ADPE [kg Sb-Eq.] 5.22E-5 5.89E-8 1.13E-6 0 4.66E-7 3.55E-7 1.88E-7 0 -9.34E-7
ADPF [MJ] 1486 12.8 57.1 0 125 60.4 79.8 0 -69.2
WDP [m³ world-Eq deprived] 18.6 6.59E-4 0.38 0 0.03 0.02 0.05 0 -8.25
GWP = Global warming potential; ODP = Depletion potential of the stratospheric ozone layer; AP = Acidification potential of land and
water; EP = Eutrophication potential; POCP = Formation potential of tropospheric ozone photochemical oxidants; ADPE = Abiotic
Legend
depletion potential for non fossil resources; ADPF = Abiotic depletion potential for fossil resources; WDP = Water (user) deprivation
potential
RESULTS OF THE LCA - INDICATORS TO DESCRIBE RESOURCE USE according to EN 15804+A2: 1 m3
C32/40 CIIIA WTT ECOPact
Indicator Unit A1-A3 A4 A5 B1 C1 C2 C3 C4 D
PERE [MJ] 65.2 0.40 1.48 0 0.20 0.08 2.14 0 -2.58
PERM [MJ] 0.70 0 0.01 0 0 0 0 0 0
PERT [MJ] 65.9 0.40 1.49 0 0.20 0.08 2.14 0 -2.58
PENRE [MJ] 1444 12.8 56.3 0 125 60.4 79.8 0 -69.2
PENRM [MJ] 49.0 0 0.97 0 0 0 0 0 0
PENRT [MJ] 1493 12.8 57.3 0 125 60.4 79.8 0 -69.2
SM [kg] 33.9 0 0.67 0 0 0 0 0 2347
RSF [MJ] 233 0 4.62 0 0 0 0 0 0
NRSF [MJ] 597 0 11.8 0 0 0 0 0 0
FW [m³] 3.15 6.09E-4 0.06 0 1.67E-3 8.32E-4 8.4E-3 0 -3.03
PERE = Use of renewable primary energy excluding renewable primary energy resources used as raw materials; PERM = Use of
renewable primary energy resources used as raw materials; PERT = Total use of renewable primary energy resources; PENRE
= Use of non-renewable primary energy excluding nonrenewable primary energy resources used as raw materials; PENRM =
Legend
Use of non-renewable primary energy resources used as raw materials; PENRT = Total use of non-renewable primary energy
resources; SM = Use of secondary material; RSF = Use of renewable secondary fuels; NRSF = Use of non-renewable secondary
fuels; FW = Use of net freshwater
9 Environmental Product Declaration Aggregate Industries – HNL2930/009 concrete, Plant Hornsey
RESULTS OF THE LCA – WASTE CATEGORIES AND OUTPUT FLOWS according to EN 15804+A2: 1 m3
C32/40 CIIIA WTT ECOPact
Indicator Unit A1-A3 A4 A5 B1 C1 C2 C3 C4 D
HWD [kg] 0.39 1.82E-3 0.01 0 7.09E-3 0.01 0.01 0 -0.03
NHWD [kg] 6.58 6.4E-3 0.15 0 0.08 0.06 0.06 0 -0.14
RWD [kg] 0.04 9.1E-5 9.91E-4 0 8.91E-4 4.26E-4 5.98E-4 0 -5.02E-4
CRU [kg] 0 0 0 0 0 0 0 0 0
MFR [kg] 0.05 0 47.2 0 0 0 2380 0 0
MER [kg] 0 0 0 0 0 0 0 0 0
EEE [MJ] 0 0 0 0 0 0 0 0 0
EET [MJ] 0 0 0 0 0 0 0 0 0
HWD = Hazardous waste disposed; NHWD = Nonhazardous waste disposed; RWD = Radioactive waste disposed; CRU =
Legend Components for reuse; MFR = Materials for recycling; MER = Materials for energy recovery; EEE = Exported electrical energy;
EEE = Exported thermal energy
RESULTS OF THE LCA – additional impact categories according to EN 15804+A2: 1 m3 C32/40 CIIIA WTT
ECOPact
Indicator Unit A1-A3 A4 A5 B1 C1 C2 C3 C4 D
PM [Disease Incidence] 3.93E-6 5.91E-8 5.63E-7 0 2.61E-6 3.68E-7 5.48E-7 0 -8.06E-7
IRP [kBq U235-Eq.] 13.7 0.06 0.48 0 0.55 0.26 1.71 0 -1.05
ETP-fw [CTUe] 512 5.76 18.9 0 41.5 29.1 15.5 0 -21.8
HTP-c [CTUh] 6.27E-8 8.9E-11 1.36E-9 0 5.42E-10 3.92E-10 2.15E-10 0 -7.75E-10
HTP-nc [CTUh] 2.7E-6 1.01E-8 6.27E-8 0 4.25E-8 5.23E-8 1.32E-8 0 -2.32E-8
SQP [-] 246 6.50 6.19 0 0.79 0.53 16.2 0 -250
PM = Potential incidence of disease due to PM emissions; IRP = Potential Human exposure efficiency relative to U235;
Legend ETPfw = Potential comparative Toxic Unit for ecosystems; HTPc = Potential comparative Toxic Unit for humans (cancerogenic);
HTPnc = Potential comparative Toxic Unit for humans (not cancerogenic); SQP = Potential soil quality index
exposure nor radioactive waste disposal in
On Global Warming Potential (GWP): underground facilities. Potential ionizing radiation
Net values are declared for all GWP indicators in A1 from the soil, radon and from some construction
– A3. The waste status of the (waste-based) fuels materials is also not measured by this indicator.
used in cement production has been verified. Gross
emissions (i.e. including CO from incineration of
2 Disclaimer 2 –for the indicators: “abiotic depletion
waste) are 301 kg CO-eq. / t (GWP-total), 301 kg
2 potential for fossil resources”, “abiotic depletion
CO-eq. / t (GWP fossil), 0.25 kg CO eq. / t (GWP-
2 2 potential for non-fossil resources”, “water (user)
biogenic).
deprivation potential”, “deprivation-weighted water
consumption”, “potential comparative toxic unit for
For wastes with biogenic carbon content, gross CO ecosystems”, “potential comparative toxic unit for
2
emissions correspond to the uptake of biogenic humans - cancer effects”, “potential comparative
CO2 during the biomass growth phase. toxic unit for humans – non-cancer effects”,
“potential soil quality index”. The results of this
environmental impact indicator shall be used with
Disclaimer 1 – for the indicator “potential Human
care as the uncertainties on these results are high
exposure efficiency relative to U235“. This impact
or as there is limited experience with the indicator.
category deals mainly with the eventual impact of
low dose ionizing radiation on human health of the
nuclear fuel cycle. It does not consider effects due
to possible nuclear accidents, occupational
10 Environmental Product Declaration Aggregate Industries – HNL2930/009 concrete, Plant Hornsey
6. LCA: Interpretation
The following table shows the most important influencing factors on important indicators of the impact and life
cycle inventory analysis.
Category GWP AP EP POCP PERT PENRT ADPE FW PM
total terrestrial
Cement 73.6 % 25.2 % 31.3 % 29.2 % 46.3 % 41.5 % 6.75 % 5.87 % 32.3 %
Aggregate 1.81 % 3.39 % 5.50 % 5.10 % 5.17 % 5.44 % 1.51 % 78.3 % 17.8 %
Cementitious 11.4 % 10.6 % 8.15 % 11.6 % 7.51 % 16.1 % 0.57 % 6.24 % 20.1 %
Fibers 0 % 0 % 0 % 0 % 0 % 0 % 0 % 0 % 0 %
Admixtures 2.54 % 1.70 % 1.72 % 2.10 % 31.0 % 9.00 % 89.6 % 1.07 % 7.06 %
Other materials
and processes 10.6 % 59.2 % 53.3 % 52.0 % 10.0 % 28.0 % 1.61 % 8.47 % 22.7 %
Total 100% 100% 100% 100% 100% 100% 100% 100% 100%
Cement: Includes the impacts for the production of all cements used. Aggregate: Includes the impacts for the production
of sand and gravel. Cementitious: Includes the impacts for the production of all cementitious materials used such as
Legend slag, fly ash or limestone. Fibers: Includes the impacts for the production of fibers. Admixtures: Includes the impacts for
the production of concrete admixtures such as plasticisers or retarders. Other materials and processes: Includes the
impacts of materials or production processes not covered by the above categories.
In the production of concrete, cement production materials. The contribution of other processes in the
dominates all impact categories. This applies in plant is low, especially with regard to greenhouse,
particular to the global warming potential (GWP). acidification and eutrophication impact categories.
Another major influencing factor is the
extraction/production and transport of the raw
7. Requisite evidence
7.1 Radioactivity concentrations will equate to an annual effective dose
Measurements of the specific activity (gamma of about 0.25 mSv (excess to the dose received
spectrometry) in Europe resulted in the following outdoors) (Radiation Protection 112).
typical values for concrete (Radiation Protection 112)
(in Bq/kg concrete). In United Kingdom there are currently no statutory limit
values for assessing the radioactivity of building
Element Typical values (max values) materials.
RA226 40 (240)
7.2 VOC emissions and leaching
Th228 30 (190)
The environmental compatibility of concrete is ensured
K40 400 (1600)
by the fact that only standardized starting materials
may be used that are a priori regarded as harmless.
Radiation exposure in an apartment block made of Therefore, no tests are normally carried out for VOC
concrete with the above average activity emissions and leaching of concrete.
8. References
Standards BS EN 16757:2017. Sustainability of construction
works. Environmental product declarations. Product
EN 12350 Category Rules for concrete and concrete elements
BS EN 12350-4:2019 Testing fresh concrete
EN 1992-1-2
EN 12390 BS EN 1992-1-2:2004+A1:2019, Eurocode 2. Design
BS EN 12390-3:2019 Testing hardened concrete of concrete structures - General rules. Structural fire
design
EN 13501-1
BS EN 13501-1:2018, Fire classification of EN ISO 14025
construction products and building elements - BS EN ISO 14025:2011, Environmental labels and
Classification using data from reaction to fire tests declarations. Type III environmental declarations.
Principles and procedures
EN 13501-2
BS EN 13501-2:2016 Fire classification of construction EN 15804
products and building elements. Classification using EN 15804:2012+A2+AC:2021, Sustainability of
data from fire resistance tests, excluding ventilation construction works. Environmental product
services declarations. Core rules for the product category of
construction products
EN 16757
BS 8500
11 Environmental Product Declaration Aggregate Industries – HNL2930/009 concrete, Plant Hornsey
BS 8500:2023 Concrete - Complementary British Product category rules on Guidance-Texts for Building-
Standard to BS EN 206 Related Products and Services. Part B: Requirements
on the EPD for Concrete components made of in-situ
Other literature or ready-mixed concrete, V6, Berlin: Institut Bauen und
Umwelt e.V. 17/07/2023
CarbonCLARITYTM EN 15804 EPD Generator - RMX
Version 1.0.1 dated 27/05/2024
www.climateearth.com
ECHA
European Chemicals Agency (ECHA): Candidate List
of Substances of Very High Concern for Authorization.
https://echa.europa.eu/
DEFRA
Department for Environment Food & Rural Affairs
(DEFRA), UK statistics on waste, May 2022:
Department for Environment Food & Rural Affairs
(DEFRA), UK statistics on waste, May 2022
Ecoinvent
Database, version 3.8, Ecoinvent, 2021.
EF 3.0
Environmental Footprint, ref package 3.0, November
2019 (European Platform on Life Cycle Assessment
(EPLCA))
IBU 2021
Institut Bauen und Umwelt e.V.: General instructions
for the EPD program of Institut Bauen und Umwelt e.V.
Version 2.0, Berlin: Institut Bauen und Umwelt e.V.,
2021. www.ibu-epd.com
No 528/2012
Regulation (EU) No 528/2012 of the European
Parliament and of the Council of 22 May 2012
concerning the making available on the market and
use of biocidal products
Radiation Protection 112
European Commission, Directorate-General for
Environment, Radiological protection principles
concerning the natural radioactivity of building
materials, Publications Office, 2000
REACH Regulation
Registration, Evaluation, Authorisation and Restriction
of Chemicals, EG 1907/2006:2006-12-18
WCO
Waste Catalog Ordinance (WCO), December 10th
2001
PCR Part A
Product category rules for building related products
and services. Part A: Calculation rules for the life cycle
assessment and requirements for the project report
according to EN 15804+A2:2021 (v1.3). Berlin: Institut
Bauen und Umwelt e.V., 31/08/2022
PCR Cement
Product category rules for building related products
and services. Part B: Requirements for the EPD for
cement, version 5. Berlin: Institut Bauen und Umwelt
e.V. (ed.), 04/07/2023.
www.ibu-epd.com
PCR Part B
12 Environmental Product Declaration Aggregate Industries – HNL2930/009 concrete, Plant Hornsey
Publisher
IBU - Institut Bauen und Umwelt e.V. Tel +49 (0)30 3087748 - 0
Hegelplatz 1 Fax +49 (0)30 3087748 - 29
10117 Berlin Mail info@ibu-epd.com
Germany Web www.ibu-epd.com
Programme holder
IBU - Institut Bauen und Umwelt e.V. Tel +49 (0)30 3087748 - 0
Hegelplatz 1 Fax +49 (0)30 3087748 - 29
10117 Berlin Mail info@ibu-epd.com
Germany Web www.ibu-epd.com
Author of the Life Cycle
Assessment
Climate Earth, Inc. Tel +1 (415) 391-2725
137 Park Place, Suite 204 Mail info@climateearth.com
Point Richmond, CA 94801 Web www.climateearth.com
United States
Owner of the Declaration
Aggregate Industries Tel +44 20 8380 7300
Bardon Hall Mail
LE67 1TL Coalville
United Kingdom london.concrete@aggregate.com
Web www.aggregate.com
13 Environmental Product Declaration Aggregate Industries – HNL2930/009 concrete, Plant Hornsey
