ENVIRONMENTAL PRODUCT DECLARATION
as per ISO 14025 and EN 15804+A2
Owner of the Declaration dormakaba International Holding GmbH
Publisher Institut Bauen und Umwelt e.V. (IBU)
Programme holder Institut Bauen und Umwelt e.V. (IBU)
Declaration number EPD-DOR-20230119-CBA1-EN
Issue date 13.04.2023
Valid to 12.04.2028
Concealed Door Closer ITS 96
dormakaba
www.ibu-epd.com | https://epd-online.com
General Information
dormakaba Concealed Door Closer ITS 96
Programme holder Owner of the declaration
IBU – Institut Bauen und Umwelt e.V. dormakaba International Holding GmbH
Hegelplatz 1 DORMA Platz 1
10117 Berlin 58256 Ennepetal
Germany Germany
Declaration number Declared product / declared unit
EPD-DOR-20230119-CBA1-EN 1 piece of the product: Concealed Door Closer ITS 96, consisting of the
following items:
• Concealed Door Closer ITS 96 EN 3-6
• Product Packaging
This declaration is based on the product category rules: Scope:
Building Hardware products, 01.08.2021 This Environment Product Declaration refers to a specific door closer
(PCR checked and approved by the SVR) manufactured by dormakaba. This EPD is also representing the variants
ITS 96 EN 2-4 and ITS 96 3-6 BCA. The production site is located in
Ennepetal (Germany). Green electricity is being used at this production
Issue date site.
13.04.2023
The data represents the year 2022.
The owner of the declaration shall be liable for the underlying information
and evidence; the IBU shall not be liable with respect to manufacturer
Valid to
information, life cycle assessment data and evidences.
12.04.2028
The EPD was created according to the specifications of EN 15804+A2. In
the following, the standard will be simplified as EN 15804.
Verification
The standard EN 15804 serves as the core PCR
Independent verification of the declaration and data according to ISO
14025:2011
internally X externally
Dipl.-Ing. Hans Peters
(Chairman of Institut Bauen und Umwelt e.V.)
Florian Pronold Matthias Klingler,
(Managing Director Institut Bauen und Umwelt e.V.) (Independent verifier)
1 Environmental Product Declaration - dormakaba - Concealed Door Closer ITS 96
Product
Product description/Product definition Base materials/Ancillary materials
The integrated ITS 96 slide channel door closer system is a The major material composition including the packaging of the
modular and multifunctional system comprising only with a few product is listed below:
door closer models and various slide channels which complies Name Value Unit
with many functional requirements. The dormakaba ITS 96 door
Steel 87 %
closer is designed for concealed installation in the door leaf and
Oil 4 %
frame. Suitable for almost every type of door, it offers a wide
variety of functions and flexibility combined with a high level of Paint 3 %
quality. Because of its compact design, the ITS 96 system can Paper 3 %
be concealed for virtual invisibility within the door and frame, Zinc 2 %
integrating inconspicuously with the overall architectural
Plastics 1 %
ambience.
The product/s include/s partial articles which contain
With the new integrated door closer ITS 96 EN 3-6 with substances listed in the Candidate List of REACH Regulation
hydraulic backcheck (BCA), doors cannot be thrown open in an 1907/2006/EC (date: 17.01.2023) exceeding 0.1 percentage by
uncontrolled manner, which offers effective protection against mass: yes
damage and accidents. For placing on the market in the • Lead (Pb): 7439-92-1 (CAS-No.) is included in some of
European Union/European Free Trade Association (EU/EFTA, the alloys used. The concentration of lead in each
with the exception of Switzerland), Regulation (EU) No. individual alloy does not exceed 4.0% (by mass).
305/2011 of the Construction Product Regulations (CPR) The Candidate List can be found on the ECHA website
applies. The product needs a declaration of performance taking address: https://echa.europa.eu/de/home.
into consideration the EN 1154 for door closer applicable for fire
and smoke check doors. The CE mark for building products is Reference service life
available. For the application and use the respective national The reference service life for the ITS 96 variants amount to 20
provisions apply: years and depend on the application and frequency of use. For
• EN 1154 repairs or renewals, suitable spare parts are available. The
• EN 1634-1 door closers are tested and certified to EN 1154, meaning they
are designed to withstand a minium of 500.000 cycles.
Application
The functions of the ITS 96 can be individually adapted to the
local conditions of each application. The closing strength can
be easily varied in accordance with the door width via the
adjustment screw accessible from the top. The closing speed,
the latch action and the backcheck can likewise be modified at
any time using adjustment screws at the top, even after the
door has been hung.
Technical Data
The door closers have following technical properties:
Performance data of the product with respect to its
characteristics in accordance with the relevant technical
provision which can be applied are mentioned above.
2 Environmental Product Declaration - dormakaba - Concealed Door Closer ITS 96
LCA: Calculation rules
Declared Unit End-of-life stage– Modules C1-C4 and D
The declared unit is 1 piece of the product: ITS 96. The end-of-life stage includes:
Name Value Unit — C1, de-construction, demolition:
Declared unit 1 piece/product — C2, transport to waste processing;
— C3, waste processing for reuse, recovery and/or recycling;
Mass of declared Product 2.67 kg
— C4, disposal;
including provision and all transport, provision of all materials,
System boundary
products and related energy and water use.
The type of EPD is: cradle to gate with options, modules C1–
C4, and module D (A1–A3 + C + D and additional modules: A4
Module D (Benefits and loads beyond the system boundary)
+ A5)
includes:
— D, recycling potentials, expressed as net impacts and
Production - Module A1-A3
benefits.
The product stage includes:
— A1, raw material extraction, processing andnmechanical Geographic Representativeness
treatments, processing of secondary Land or region, in which the declared product system is
material input (e.g. recycling processes), manufactured, used or handled at the end of the product´s
— A2, transport to the manufacturer, lifespan: Global
— A3, manufacturing and assembly including provision of all
materials, products and energy, as well as waste processing up
to the end-of waste state. Comparability
Basically, a comparison or an evaluation of EPD data is only
Construction stage - Modules A4-A5 possible if all the data sets to be compared were created
The construction process stage includes: according to EN 15804 and the building context, respectively
— A4, transport to the building site; the product-specific characteristics of performance, are taken
— A5, installation into the building; into account.
including provision of all materials, products and energy, as well
as waste processing up to the end-of waste state or disposal of
final residues during the construction process stage.
LCA: Scenarios and additional technical information
Installation into the building (A5)
Characteristic product properties of biogenic carbon
Name ValueUnit
Output substances following waste treatment on
Information on describing the biogenic Carbon Content at 0.07 kg
site (packaging)
factory gate
Name ValueUnit
Biogenic carbon content in accompanying kg End of life (C1-C4)
0.03
packaging C C1: The product dismantling from the building is done manually
without environmental burden.
C2: Transport to waste treatment at end of life is 50 km.
Name Value Unit
Transport to the building site (A4) Collected separately waste type 2.6 kg
Recycling 2.58 kg
Name Value Unit
Energy recovery 0.022 kg
Litres of fuel truck (per piece) 0.008l/100km
Transport distance via truck (for scaling) 100 km Reuse, recovery and/or recycling potentials (D), relevant
Transport distance via truck (from dormakaba scenario information
300 km
logistic center to harbor)
Name Value Unit
Capacity utilisation (including empty runs)
55 % Recycling 100 %
average
The collection rate is 100%.
Transport distance via ship 11000 km
The product is transported via truck and ship. The product is
stored in the dormakaba logistic center in Germany. The main
distribution regions are Europe and Asia. In order to allow
scaling to a specific point of installation 100 km are declared as
well.
3 Environmental Product Declaration - dormakaba - Concealed Door Closer ITS 96
LCA: Results
DESCRIPTION OF THE SYSTEM BOUNDARY (X = INCLUDED IN LCA; ND = MODULE OR INDICATOR NOT DECLARED; MNR =
MODULE NOT RELEVANT)
Benefits and
Construction loads beyond
Product stage Use stage End of life stage
process stage the system
boundaries
la ire ta m w a Ry lp p u s tro p s n a rT g n iru tc a fu n a M e h t m o rf tro p s n a rTe tis e h t o t e ta g y lb m e s s A e s U e c n a n e tn ia M ria p e R tn e m e c a lp e R tn e m h s ib ru fe R y g re n e la n o ita re p Oe s u re ta w la n o ita re p Oe s u n o itc u rts n o c -e Dn o itilo m e d tro p s n a rT g n is s e c o rp e ts a W la s o p s iD -e s u e R-y re v o c e R-g n ilc y c e Rla itn e to p
A1 A2 A3 A4 A5 B1 B2 B3 B4 B5 B6 B7 C1 C2 C3 C4 D
X X X X X MND MND MNR MNR MNR MND MND X X X X X
RESULTS OF THE LCA - ENVIRONMENTAL IMPACT according to EN 15804+A2: 1 door closer
Parameter Unit A1-A3 A4 A5 C1 C2 C3 C4 D
GWP-total kg CO 2 eq 4.45E+00 1.89E-01 1.03E-01 0 1.14E-02 5.24E-01 0 -1.4E+00
GWP-fossil kg CO 2 eq 4.58E+00 1.85E-01 2.59E-03 0 1.09E-02 5.14E-01 0 -1.4E+00
GWP-biogenic kg CO 2 eq -1.34E-01 4.25E-03 1.01E-01 0 5.02E-04 1.08E-02 0 -2.76E-03
GWP-luluc kg CO 2 eq 4.6E-03 4.1E-06 1.7E-06 0 2.58E-07 2.91E-05 0 -2.68E-04
ODP kg CFC11 eq 7.16E-12 1.85E-17 1.87E-17 0 1.15E-18 2.6E-16 0 -1.43E-12
AP mol H+ eq 1.41E-02 3.63E-03 2.9E-05 0 1.09E-05 9.3E-05 0 -3.46E-03
EP-freshwater kg P eq 1.15E-05 4.07E-08 3.65E-09 0 2.32E-09 4.15E-08 0 -1.27E-06
EP-marine kg N eq 2.7E-03 9.62E-04 1.05E-05 0 3.46E-06 2.11E-05 0 -5.99E-04
EP-terrestrial mol N eq 2.88E-02 1.05E-02 1.3E-04 0 3.84E-05 4.24E-04 0 -6.24E-03
kg NMVOC
POCP 8.75E-03 2.69E-03 2.77E-05 0 9.78E-06 5.84E-05 0 -2.22E-03
eq
ADPE kg Sb eq 3.3E-04 5.14E-09 2.95E-10 0 3.26E-10 3.57E-09 0 -6.93E-05
ADPF MJ 6.04E+01 2.43E+00 3.27E-02 0 1.54E-01 2.4E-01 0 -1.6E+01
m3 world eq
WDP 6.39E-01 3.48E-04 1.28E-02 0 2.13E-05 5.36E-02 0 -1.22E-01
deprived
GWP = Global warming potential; ODP = Depletion potential of the stratospheric ozone layer; AP = Acidification potential of land and water; EP =
Eutrophication potential; POCP = Formation potential of tropospheric ozone photochemical oxidants; ADPE = Abiotic depletion potential for non-fossil
resources; ADPF = Abiotic depletion potential for fossil resources; WDP = Water (user) deprivation potential)
RESULTS OF THE LCA - INDICATORS TO DESCRIBE RESOURCE USE according to EN 15804+A2: 1 door closer
Parameter Unit A1-A3 A4 A5 C1 C2 C3 C4 D
PERE MJ 2.78E+01 7.8E-03 8.82E-01 0 4.86E-04 1.34E-01 0 -2.01E+00
PERM MJ 9.48E-01 0 -8.76E-01 0 0 -7.2E-02 0 0
PERT MJ 2.87E+01 7.8E-03 5.94E-03 0 4.86E-04 6.23E-02 0 -2.01E+00
PENRE MJ 6.01E+01 2.43E+00 3.27E-02 0 1.54E-01 6.27E-01 0 -1.6E+01
PENRM MJ 3.87E-01 0 0 0 0 -3.87E-01 0 0
PENRT MJ 6.05E+01 2.43E+00 3.27E-02 0 1.54E-01 2.4E-01 0 -1.6E+01
SM kg 2.01E+00 0 0 0 0 0 0 0
RSF MJ 0 0 0 0 0 0 0 0
NRSF MJ 0 0 0 0 0 0 0 0
FW m3 2.9E-02 1.41E-05 3.02E-04 0 8.71E-07 1.28E-03 0 -5.53E-03
PERE = Use of renewable primary energy excluding renewable primary energy resources used as raw materials; PERM = Use of renewable primary
energy resources used as raw materials; PERT = Total use of renewable primary energy resources; PENRE = Use of non-renewable primary energy
excluding non-renewable primary energy resources used as raw materials; PENRM = Use of non-renewable primary energy resources used as raw
materials; PENRT = Total use of non-renewable primary energy resources; SM = Use of secondary material; RSF = Use of renewable secondary fuels;
NRSF = Use of non-renewable secondary fuels; FW = Use of net fresh water
RESULTS OF THE LCA – WASTE CATEGORIES AND OUTPUT FLOWS according to EN 15804+A2:
1 door closer
Parameter Unit A1-A3 A4 A5 C1 C2 C3 C4 D
HWD kg 1.02E-07 2.37E-10 4.82E-11 0 1.5E-11 9.09E-10 0 -9.4E-07
NHWD kg 2.55E-01 2.49E-04 3.24E-03 0 1.58E-05 5.34E-02 0 3.7E-02
RWD kg 2.71E-03 2.66E-06 1.72E-06 0 1.65E-07 8.97E-06 0 -7.07E-04
CRU kg 0 0 0 0 0 0 0 0
MFR kg 0 0 0 0 0 2.39E+00 0 0
MER kg 0 0 0 0 0 0 0 0
EEE MJ 0 0 1.57E-01 0 0 9.67E-01 0 0
EET MJ 0 0 2.84E-01 0 0 2.21E+00 0 0
4 Environmental Product Declaration - dormakaba - Concealed Door Closer ITS 96
HWD = Hazardous waste disposed; NHWD = Non-hazardous waste disposed; RWD = Radioactive waste disposed; CRU = Components for re-use;
MFR = Materials for recycling; MER = Materials for energy recovery; EEE = Exported electrical energy; EET = Exported thermal energy
RESULTS OF THE LCA – additional impact categories according to EN 15804+A2-optional:
1 door closer
Parameter Unit A1-A3 A4 A5 C1 C2 C3 C4 D
Disease
PM 1.92E-07 6.09E-08 1.61E-10 0 5.71E-11 1.17E-09 0 -4.89E-08
incidence
IR kBq U235 eq 3.52E-01 3.81E-04 2.66E-04 0 2.36E-05 8.17E-04 0 -1.08E-01
ETP-fw CTUe 2.27E+01 1.72E+00 1.55E-02 0 1.09E-01 9.04E-02 0 -2.71E+00
HTP-c CTUh 4.54E-09 3.23E-11 8.2E-13 0 2.05E-12 7.8E-12 0 7.03E-10
HTP-nc CTUh 1.92E-07 1.46E-09 3.55E-11 0 8.78E-11 7.85E-10 0 5.22E-08
SQP SQP 2.61E+01 6.35E-03 8.66E-03 0 3.96E-04 7.19E-02 0 -6.63E-01
PM = Potential incidence of disease due to PM emissions; IR = Potential Human exposure efficiency relative to U235; ETP-fw = Potential comparative
Toxic Unit for ecosystems; HTP-c = Potential comparative Toxic Unit for humans (cancerogenic); HTP-nc = Potential comparative Toxic Unit for humans
(not cancerogenic); SQP = Potential soil quality index
Disclaimer 1 – for the indicator “Potential Human exposure efficiency relative to U235”. This impact category deals mainly with the
eventual impact of low-dose ionizing radiation on human health of the nuclear fuel cycle. It does not consider effects due to possible
nuclear accidents, occupational exposure or radioactive waste disposal in underground facilities. Potential ionizing radiation from the
soil, radon and from some construction materials is also not measured by this indicator.
Disclaimer 2 – for the indicators “abiotic depletion potential for non-fossil resources”, “abiotic depletion potential for fossil resources”,
“water (user) deprivation potential, deprivation-weighted water consumption”, “potential comparative toxic unit for ecosystems”,
“potential comparative toxic unit for humans – cancerogenic”, “Potential comparative toxic unit for humans - not cancerogenic”,
“potential soil quality index”. The results of this environmental impact indicator shall be used with care as the uncertainties on these
results are high as there is limited experience with the indicator.
This EPD was created using a software tool.
References
EN 1154 GaBi ts documentation
EN 1154-2003; Building hardware - Controlled door closing GaBi life cycle inventory data documentation (https://www.gabi-
devices - Requirements and test methods software.com/support/gabi/gabidatabase-2020-lci-
documentation/)
EN 1634-1
EN 1634-1:2018-04; Fire resistance and smoke control tests for IBU
door and shutter assemblies, openable windows and elements Institut Bauen und Umwelt e.V.: General Instructions for the
of building hardware - Part 1: Fire resistance test for door and EPDs programme of Institut Bauen und Umwelt e.V. Version
shutter assemblies and openable windows 2.0., Berlin: Institut Bauen und Umwelt e.V., 2021. www.ibu-
epd.com
EN 15804
EN 15804+A2:2019+AC:2021, Sustainability of construction LCA-tool dormakaba
works — Environmental Product Declarations — Core rules for LCA tool IBU-DOR-202104-LT1-EN, version 1.0, 2021.
the product category of construction products Developed by Sphera Solutions GmbH
ISO 14025 PCR Part A
DIN EN ISO 14025:2011-10, Environmental labels and PCR – Part A: Calculation Rules for the Life Cycle Assessment
declarations — Type III environmental declarations — and Requirements on the Project Report according to EN
Principles and procedures 15804+A2:2019, Version 1.0, 2020, Institut Bauen und Umwelt
e.V., www.ibu-epd.com
ECHA
European Chemicals Agency: https://echa.europa.eu/de/home PCR Part B
PCR – Part B: Requirements on the EPD for Building Hardware
REACH product, version 1.2, Institut Bauen und Umwelt e.V., www.ibu-
Registration, Evaluation, Authorisation and Restriction of epd.com, 2017
Chemicals (REACH), Regulation (EC) No 1907/2006
Further References
GaBi
Sphera Solutions GmbH Gabi Software System and Database
for Life Cycle Engineering 1992-2020 Version 10.0.0.71
University of Stuttgart Leinfelden-Echterdingen
5 Environmental Product Declaration - dormakaba - Concealed Door Closer ITS 96
Publisher
Institut Bauen und Umwelt e.V. +49 (0)30 3087748- 0
Hegelplatz 1 info@ibu-epd.com
10117 Berlin www.ibu-epd.com
Germany
Programme holder
Institut Bauen und Umwelt e.V. +49 (0)30 3087748- 0
Hegelplatz 1 info@ibu-epd.com
10117 Berlin www.ibu-epd.com
Germany
Author of the Life Cycle Assessment
dormakaba International Holding GmbH +49 2333 793-0
DORMA Platz 1 info.de@dormakaba.com
58256 Ennepetal www.dormakaba.com
Germany
Owner of the Declaration
dormakaba International Holding GmbH +49 2333 793-0
DORMA Platz 1 info.de@dormakaba.com
58256 Ennepetal www.dormakaba.com
Germany
6 Environmental Product Declaration - dormakaba - Concealed Door Closer ITS 96
