LOGO OF THE EPD’S OWNER]
DAPH ABITAT S YSTEM E NVIRONMENTAL P RODUCT D ECLARATION
WWW.DAPHABITAT.PT [ACCORDING TO ISO 14025, EN 15804:2012+A2:2019 AND EN 15942]
Declaration number: DAP 011:2024
ISAC1 - INERT STEEL AGGREGATES FOR CONSTRUCTION
ISSUE DATE: 04/10/2024 VALID UNTIL: 03/10/2024
SIDERURGIA NACIONAL, EMPRESA DE PRODUTOS LONGOS, S.A.
Version 1.4. Ed. March 2024
1 ASIC in Portuguese (Agregado Siderúrgico Inerte para a Construção)
1
INDEX
1. GENERAL INFORMATION .................................................................................................................................... 1
1.1. The DAPHAbitat System .............................................................................................................................................. 1
1.2. EPD owner ................................................................................................................................................................... 1
1.3. Information concerning the EPD ................................................................................................................................. 2
1.4. Demonstration of the verification ............................................................................................................................... 2
1.5. EPD Registration .......................................................................................................................................................... 2
1.6. PCR (product category rules) basic model ................................................................................................................... 3
1.7. Relevant c-PCR (Complementary product category rules) .......................................................................................... 3
1.8. Information concerning the product/product class .................................................................................................... 4
1.9. Calculation rules of the LCA ......................................................................................................................................... 5
1.10. Use of average environmental performance ............................................................................................................... 6
1.11. Technical information for Reference Service Life (RSL) ............................................................................................... 6
1.12. Flow diagram of input and output of the processes.................................................................................................... 7
2. CORE ENVIRONMENTAL IMPACT INDICATORS ......................................................................................................... 8
2.1. Description of the system boundaries ......................................................................................................................... 8
2.1.1. Justification for the exemption to declare modules C1, C2, C3, C4 and D ............................................................ 8
2.2. Core environmental impact indicators ........................................................................................................................ 9
2.3. Additional environmental impact indicators ............................................................................................................. 10
2.4. Indicators describing resource use ............................................................................................................................ 11
2.5. Other environmental information describing different waste categories ................................................................ 12
2.6. Environmental information describing output flows ................................................................................................ 12
2.7. Information describing the biogenic carbon content at the factory gate ................................................................. 12
3. SCENARIOS AND ADDITIONAL TECHNICAL INFORMATION ...................................................................................... 13
3.1. C2 Transport – End-of-life of the product ................................................................................................................. 13
3.2. C3 Waste processing for reuse. recovery and/or recycling – End-of-life of the product .......................................... 13
3.3. C4 Disposal – End-of-life of the product .................................................................................................................... 13
3.4. Scenario and technical information for module D..................................................................................................... 13
3.5. Additional information on release of dangerous substances to indoor air, soil, and water during the use stage .... 13
4. REFERENCES ....................................................................................................................................................... 14
SISTEMA DAPHABITAT iii
1. GENERAL INFORMATION
1.1. The DAPHabitat System
Sustainable Construction Platform
Program operator: www.clusterhabitat.pt
geral@clusterhabitat.pt
Departamento Engenharia Civil
Address: Universidade de Aveiro
3810-193 Aveiro
Email address: deptecnico@clusterhabitat.pt
Telephone number: (+351) 234 401576
Website: www.daphabitat.pt
Logo
1.2. EPD owner
Name of the owner: Siderurgia Nacional – Empresa de Produtos Longos, S.A.
Maia unit: Rua da Siderurgia, 4425-514 S. Pedro Fins, Maia, Portugal
Production site:
Seixal unit: Avenida da Siderurgia Nacional, 2840-075 Aldeia de Paio Pires, Seixal, Portugal
Address (head office): Seixal unit: Apartado 3, 2840-996 Aldeia de Paio Pires, Seixal, Portugal
Maia unit: (+351) 229 699 000
Telephone:
Seixal unit: (+351) 212 278 500
E-mail: efraguela@megasa.pt; acanelas@megasa.pt
Website: www.megasa.com
Logo:
Information concerning the
Both production premises have Environmental License and Management Systems implemented
applicable management
according to ISO 9001, ISO 14001, ISO 45001, ISO 50001 and Steel Sustainability.
Systems:
Specific aspects regarding Main CAE 24100 – Steelmaking and elaboration of ferro-alloys
the production: Secondary CAE 38322 – Valorisation of non-metallic wastes
Siderurgia Nacional – Empresa de Produtos Longos, S.A. is aware that the activity must be performed in
a way that guarantees the achievement of the highest levels of protection for the people working in
the premises, the sustainability and continuous growth of the company, the highest levels of quality in
Organization’s
products and services and the maximisation of eco-efficiency, through the continual improvement of
environmental policy:
management and performance in the fields of Health and Safety, Sustainability, Quality, Environment
and Major Risk Prevention involving dangerous substances. The complete integrated policies of both
Maia and Seixal units are available on the website www.megasa.com.
DAPHabitat System 1
1.3. Information concerning the EPD
Authors: Ana Cláudia Dias
Contact of the authors: Address: University of Aveiro, Campus Universitário de Santiago, 3810-193 Aveiro, Portugal
Phone number: +351 234 370 200
E-mail: acdias@ua.pt
Issue date: 04/10/2024
Registration date: 22/10/2024
Registration number: DAP 011:2024
Valid until: 03/10/2029
Representativity of the EPD
(location, manufacturer, EDP of one (1) product prepared in two (2) industrial units, pertaining to two (2) producers.
group of manufacturers):
Where to consult
www.megasa.com
explanatory material:
Type of EPD: Cradle-to-gate EDP (A1-A3) with modules C and D
1.4. Demonstration of the verification
External independent verification, accordingly with the standard ISO 14025:2010 and EN 15804:2012+A2:2019
Certification Body Verifier
(CERTIF – Associação para a Certificação) (Marisa Almeida)
1.5. EPD Registration
Programme operator
(Plataforma para a Construção Sustentável)
DAPHabitat System 2
1.6. PCR (product category rules) basic model
Name: PCR: Basic module for construction products and services
Issue date: Edition August 2023
Number of registration on the data
RCP-mb001
base:
Version: Version 2.3
Marisa Almeida | marisa@ctcv.pt
Identification and contact of the
Luís Arroja | arroja@ua.pt
coordinator (s):
José Dinis Silvestre | jose.silvestre@ist.utl.pt
Marisa Almeida | marisa@ctcv.pt
Identification and contact of the
Luís Arroja | arroja@ua.pt
authors:
José Silvestre | jds@civil.ist.utl.pt
Fausto Freire
Cristina Rocha
Ana Paula Duarte
Ana Cláudia Dias
Helena Gervásio
Victor Ferreira
Ricardo Mateus
António Baio Dias
Composition of the Sectorial Panel: -
Consultation period: 18/11/2015 - 18/01/2016
Valid until: 01/06/2027
CEN standard EN 15804 serves as the core Product Category Rules (PCR).
1.7. Relevant c-PCR (Complementary product category rules)
Not applicable.
DAPHabitat System 3
1.8. Information concerning the product/product class
Identification of the product: ISAC - Inert Steel Aggregates for Construction
Illustration of the product:
Brief description of the product: ISAC is a product obtained after treating the slag that result from EAF (electric arc
furnace) steelmaking. ISAC is sold in several particle sizes and this EPD is valid for
aggregate dimensions of 0-40 mm (ISAC 0-40), 40-100 mm (ISAC 40-100), 0-6 mm (ISAC 0-
6), 6-12 mm (ISAC 6-12) and 10-16 mm (ISAC 12-18).
Main technical characteristics of the The technical characteristics of ISAC comply with the requirements of the following
product: Standards: EN 13242 – Aggregates for unbound and hydraulically bound materials for use
in civil engineering work and road construction, EN 12620 – Aggregates for concrete, and
EN 13043 – Aggregates for bituminous mixtures and surface treatments for roads,
airfields and other trafficked areas.
Description of the product’s • Basic layers, sub-layer, road surface and landfilling for roads;
application/use: • Landfilling layers, upper layer and sub-ballast for railway lines;
• Drainage layers;
• Accesses, machine parks and building site pavement;
• Aggregates for concrete.
Placing on the market / Rules of ISAC is marketed in bulk and subject to CE-marking according to the following Standards:
application in the market / Technical EN 13242 – Aggregates for unbound and hydraulically bound materials for use in civil
rules of the product: engineering work and road construction, EN 12620 – Aggregates for concrete, and EN
13043 – Aggregates for bituminous mixtures and surface treatments for roads, airfields
and other trafficked areas.
Quality control: ISAC is subject to a Certificate of Conformity for the factory production control, thus to
external quality control regarding the compliance of EN 13242, ANNEX C, EN 12620, and
EN 13043.
Special delivery conditions: In bulk.
Components and substances to declare: Not applicable.
Where explanatory material may be
www.megasa.com
obtained:
History of the LCA studies: Not applicable.
DAPHabitat System 4
1.9. Calculation rules of the LCA
Functional unit: Not applicable.
Declared unit: 1 tonne (t) of ISAC.
System boundaries: The assessed system includes modules A1-A3 (product stage), C (end-of-life stage), and D
(benefits and loads beyond the system boundary). In the end-of-life stage, the impacts of
module C1 (deconstructions and demolition) were excluded due to the lack of information.
The raw material of ISAC is EAF slag produced during the steelmaking process. This slag is a
waste and, thus, all processes upstream its valorisation are excluded from the system
boundaries.
During slag processing, the metallic fraction is separated and reintroduced in the
steelmaking process. This is considered as a closed-cycle valorisation system of metallic
fraction and, thus, this valorisation process has been excluded from the system boundaries
but the transportation of metallic fraction up to the valorisation site is considered.
Most of the water consumed during ISAC production process comes from industrial purges;
thus, its collection and treatment have not been considered.
A more detailed description of the system boundary is presented in Section 2.1.
Criteria for the exclusion: The LCA considered all the production processes of the materials and energy consumed in
the system, as well as the management processes of the wastes generated, for which
inventory data were available. The flows of materials and wastes excluded in the ISAC
production process (absorbent rags, oil filters, wastes from sewer cleaning, and wastes from
oil/water separators) are much lower than 1% of the total mass of the inputs to that process
and 5% of the total mass of inputs to the respective information module (cut-off criteria
defined in EN 15804).
The consumption of energy and water in the administrative areas and workshops, as well as
the production of wastewater and wastes from these areas, were excluded. The
environmental burdens from the construction and maintenance of infrastructures and
equipment (capital goods) were also excluded, except those associated with the
maintenance of machinery and vehicles used in the production of ISAC.
Assumption and limitations The results of the environmental impacts and remaining indicators shown in this EDP refer
to the year 2022 and constitute weighted average values based on the amount of ISAC
produced by each production unit that year (49.5% in Seixal and 50.5% in Maia).
Quality and other characteristics In the case of processes on which the producer has influence (slag preparation and
about the information used in the processing), real and specific data collected in both production units have been used. The
LCA: exception are emissions to air resulting from diesel combustion in lorries and machines used
during internal operations of transport and transference and from propane combustion in
welding operations, which have been calculated with emission factors due to the lack of
measured values.
For the remaining processes, except for ferrous metals recycling considered in module D,
generic data obtained from the Ecoinvent - version 3.9.1 database have been used, which
meet the quality criteria defined for generic data (time-related, geographical and
technological representativeness, plausibility, completeness, consistency, etc.).
Data for ferrous metals recycling considered in module D were retrieved from an EPD for
hot-rolled ribbed steel proceeding from an electric arc furnace produced in four Megasa
plants (https://www.en.aenor.com/Producto_DAP_pdf/MEGASA_001-007.pdf).
According to the criteria defined in Table E.1 of Annex E of the EN 15804 standard, defined
by “UN Environment Global Guidance on LCA database development”, the quality of
relevant data and data used in module D is very good for both technological and temporal
representativeness, and is good for the geographical representativeness, except for the
production of electricity, for which it is considered very good.
Allocation rules: The production of ISAC with different particle sizes occurs simultaneously and their
environmental impacts cannot be obtained individually. Thus, the results obtained are valid
for all particle sizes.
Software used for the assessment: SimaPro version 9.5.0.2.
Background database used for the Ecoinvent version 3.9.1 database published in December 2022; “cut-off” approach.
LCA:
Comparability of EPD for construction The EPD of construction products and services cannot be comparable in case they are not
products produced according to EN 15804 and EN 15948 and according to the comparability
conditions determined by ISO 14025.
DAPHabitat System 5
1.10. Use of average environmental performance
This EPD presents the average environmental performance of all particle sizes of ISAC produced by Siderurgia
Nacional – Empresa de Produtos Longos, S.A. at the Seixal and Maia plants. For the core environmental impacts
indicators, in the module A1-A3, the variability of the individual impacts of each production plant compared to the
average values reported in this EPD ranges from 1 to 22%. In eight out of the thirteen core indicators this
variability does not exceed 3%. In the module D, the variability of the individual core environmental impacts of
each production plant compared to the average values does not exceed 0.6%.
1.11. Technical information for Reference Service Life (RSL)
Not applicable.
DAPHabitat System 6
1.12. Flow diagram of input and output of the processes
Figure 1: Life cycle stages and unit processes.
DAPHabitat System 7

DRR
A 1 - e x tra c tio n a n d p ro c e s s in g o f ra w m
A 2 - tra n s p o r t
A 3 - m a n u fa c tu r in g
S la g p re p a ra tio n
S la g c o lle c tio n
T ra n sp o rt to c o o lin g a re a
C o o lin g
T ra n sp o rt to p ro c e ssin g a re a
S la g p ro c e s s in g
C o o lin g
S e p a ra tio n o f m e ta llic c o m p o n e n t a n d fra g m
S e p a ra tio n b y p a rtic le size
IS A C sto ra g e
IS A C sh ip m e n t
IS A C
C - e n d o f life
C 2 : tra n sp o rt
C 3 : w a ste p ro c e ssin g
C 4 : w a ste d isp o sa l
- b e n e fits a n d lo a d s b e y o n d th e s y s te me
u se o f IS A C a t th e e n d o f lifee
c y c lin g o f fe rro u s m e ta ls fro m IS A C p ro d u c tio
S y s te m
a te r ia ls
e n ta tio n
b o u n d a r y
n
b o u n d a r ie s
Mv
R
a
e
a te ria ls folo
ris a tio n
u s e o f IS A
r
C
2. CORE ENVIRONMENTAL IMPACT INDICATORS
2.1. DESCRIPTION OF THE SYSTEM BOUNDARIES
(✓= included; ND = module not declared)
BENEFITS AND LOADS
CONSTRUCTION
PRODUCT STAGE USE STAGE END-OF-LIFE STAGE BEYOND THE SYSTEM
PROCESS STAGE
BOUNDARY
la
y lp p u s la ire ta m w a R tro p s n a rT g n iru tc a fu n a M tro p s n a rT s s e c o rp n o ita lla ts n i n o itc u
rts
e s U e c n a n e tn ia M ria p e R tn e m e c a lp e R tn e m h s ib ru fe R e s u y g re n e la n o ita re p O e s u re ta w la n o ita re p O n o itilo m e d ,s n o itc u rts n eo Dc - tro p s n a rT g n is s e c o rp e ts a W la s o p s iD
itn
e to p g n ilc y c e r ,y re v o c e r ,e
s
u
n o
C
e R-
A1 A2 A3 A4 A5 B1 B2 B3 B4 B5 B6 B7 C1 C2 C3 C4 D
✓ ✓ ✓ ND ND ND ND ND ND ND ND ND ND ✓ ✓ ✓ ✓
The product stage (module A1-A3) considers the manufacturing of ISAC, as well as the extraction, processing, and transport of
materials and energy vectors, and also waste processing until its end-of-life. ISAC production is divided into two processes: slag
preparation and slag processing. Slag preparation starts with EAF slag collection for its solidification in the specific area so-
called slag pit. Then, slag is transported to the water-cooling area, to be transported to the processing area after cooling.
During slag processing, it is cooled with water, with the further separation of metallic components and slag fragmentation. Slag
is submitted to the following operations: (1) separation by sieving/calibration in particle size fractions appropriate for the
different applications; (2) new mechanical fragmentation, eventually with a grinding operation for a better inclusion of fine
particles and the increase of smaller particle sizes; (3) elimination of the smallest metallic chips which were not eliminated
before. Then ISAC is stored outdoors. Finally, lorries are loaded for dispatch.
In the end-of-life stage, the impacts from module C1 (deconstruction and demolition) were excluded because, although
mechanised deconstruction and demolition of structures containing ISAC may occur, there is no information available allowing
the quantification of the respective impacts. The following submodules were considered:
• C2 (transport): ISAC is assumed to be reused in the same place and, thus, no transport is required;
• C3 (waste processing): ISAC reuse does not require any additional processing;
• C4 (waste disposal): ISAC is reused and, therefore, does not undergo final disposal processes.
Module D considers the environmental benefits and loads associated with ISAC reuse at the end-of-life (replacing gravel) and
with ferrous metals scrap generated in the ISAC manufacturing process that is recycled.
2.1.1. Justification for the exemption to declare modules C1, C2, C3, C4 and D
Not applicable.
DAPHabitat System 8
2.2. Core environmental impact indicators
Depletion
Global Global warming
Global warming Global warming potential of the
warming potential fossil; potential biogenic; potential land use stratospheric Acidification
potential total; and land use change; ozone layer; potential; AP
GWP-fossil GWP-biogenic
GWP-total GWP-luluc
ODP
Unit kg CO2 eq. kg CO2 eq. kg CO2 eq. kg CO2 eq. kg CFC 11 eq. mol H+ eq.
Module A1-A3 7.49E+00 7.36E+00 1.28E-01 8.52E-03 1.61E-07 4.78E-02
Module C2 0.00E+00 0.00E+00 0.00E+00 0.00E+00 0.00E+00 0.00E+00
Module C3 0.00E+00 0.00E+00 0.00E+00 0.00E+00 0.00E+00 0.00E+00
Module C4 0.00E+00 0.00E+00 0.00E+00 0.00E+00 0.00E+00 0.00E+00
Module D -3.26E+00 -3.11E+00 -1.30E-01 -1.63E-02 -5.53E-08 -2.17E-02
LEGEND:
Product stage
End-of-life stage
Benefits and loads beyond the system boundary
Values expressed per declared unit (1 t of ISAC).
Eutrophication Abiotic Abiotic
Eutrophication Formation
p ao qt uen att ii ca l potential Eu ptr oo tp eh nic ta iati lo n potential of pod te ep nle tit aio l fn o r pod te ep nle tit aio l fn o r W dea pte rir v ( au ts ioe nr)
freshwater; aquatic terrestrial; tropospheric non-fossil fossil potential;
marine; ozone; resources resources
EP- EP-terrestrial potential WDP
EP-marine POCP ADP-
freshwater minerals&metals ADP-fossil
m3 World eq.
Units kg P eq. kg N eq. mol N eq. Kg COVNM eq. kg Sb eq. MJ. P.C.I
deprived
Module A1-A3 1.74E-05 2.17E-02 2.36E-01 7.46E-02 1.77E-06 1.01E+02 6.38E-01
Module C2 0.00E+00 0.00E+00 0.00E+00 0.00E+00 0.00E+00 0.00E+00 0.00E+00
Module C3 0.00E+00 0.00E+00 0.00E+00 0.00E+00 0.00E+00 0.00E+00 0.00E+00
Module C4 0.00E+00 0.00E+00 0.00E+00 0.00E+00 0.00E+00 0.00E+00 0.00E+00
Module D -4.98E-05 -7.41E-03 -8.11E-02 -2.54E-02 -7.49E-07 -4.18E+01 -5.47E+01
LEGENDA:
Product stage
End-of-life stage
Benefits and loads beyond the system boundary
Values expressed per declared unit (1 t of ISAC).
The results obtained for the indicators “Abiotic depletion potential for non-fossil resources (ADP-minerals&metals)”, “Abiotic depletion potential for fossil
resources potential (ADP-fossil)” and “Water (user) deprivation potential (WDP)” should be used with caution since the uncertainties associated with them are
high or there is little experience with the indicator.
DAPHabitat System 9
2.3. Additional environmental impact indicators
Potential Potential Potential Potential Potential
incidence of Human Comparative
Comparative Comparative Toxic Potential soil
disease due exposure Toxic Unit for
Toxic Unit for Unit for humans. quality index
to PM efficiency humans. not
ecosystems cancer effects
emissions relative to U235 cancer effects SQP
PM IRP ETP-fw HTP-c HTP-nc
Disease
Unit kBq U 235 eq. CTUe CTUh CTUh -
incidence
Module A1-A3 ND ND ND ND ND ND
Module C2 ND ND ND ND ND ND
Module C3 ND ND ND ND ND ND
Module C4 ND ND ND ND ND ND
Module D ND ND ND ND ND ND
LEGEND:
Product stage
End-of-life stage
Benefits and loads beyond the system boundary
ND - not declared.
The impact indicator “POTENTIAL HUMAN EXPOSURE EFFICIENCY RELATIVE TO U235” focuses mainly on the possible impact of a low dose of ionising
radiation on human health resulting from the nuclear fuel cycle. It does not consider effects arising from possible nuclear accidents. occupational
exposure or the disposal of radioactive waste in underground facilities. Potential ionising radiation from soil. radon and some building materials is also
not measured by this indicator.
The results of the indicators “POTENTIAL COMPARATIVE TOXIC UNIT FOR ECOSYSTEMS (ETP-FW)”. “POTENTIAL COMPARATIVE TOXIC UNIT FOR
HUMANS. CANCER EFFECTS”. “POTENTIAL COMPARATIVE TOXIC UNIT FOR HUMANS. NOT CANCER EFFECTS” and “POTENTIAL SOIL QUALITY INDEX”
should be used with caution as the uncertainties associated with them are high or there is little experience with the indicator.
DAPHabitat System 10
2.4. Indicators describing resource use
Primary energy
EPR RR TRR EPNR RNR TRNR
Unit MJ. P.C.I. MJ. P.C.I. MJ. P.C.I. MJ. P.C.I. MJ. P.C.I. MJ. P.C.I.
Module A1-A3 6.21E+00 0.00E+00 6.21E+00 9.37E+01 6.93E+00 1.01E+02
Module C2 0.00E+00 0.00E+00 0.00E+00 0.00E+00 0.00E+00 0.00E+00
Module C3 0.00E+00 0.00E+00 0.00E+00 0.00E+00 0.00E+00 0.00E+00
Module C4 0.00E+00 0.00E+00 0.00E+00 0.00E+00 0.00E+00 0.00E+00
Module D -1.25E+01 0.00E+00 -1.25E+01 -4.20E+01 2.53E-01 -4.18E+01
LEGEND:
Product stage
End-of-life stage
Benefits and loads beyond the system boundary
EPR = use of renewable primary energy excluding renewable primary energy resources used as raw materials; RR = use of renewable primary energy
resources used as raw materials; TRR = total use of renewable primary energy resources (EPR + RR); EPNR = use of non-renewable primary energy
excluding non-renewable primary energy resources used as raw materials; RNR = use of non-renewable primary energy resources used as raw
materials; TRNR = total use of non-renewable primary energy resources (EPRN + RNR).
Values expressed per declared unit (1 t of ISAC).
Secondary materials and fuels, and use of water
MS CSR CSNR Net use of fresh water
Unit kg MJ. P.C.I. MJ. P.C.I. m3
Module A1-A3 1.01E+03 0.00E+00 0.00E+00 1.54E-02
Module C2 0.00E+00 0.00E+00 0.00E+00 0.00E+00
Module C3 0.00E+00 0.00E+00 0.00E+00 0.00E+00
Module C4 0.00E+00 0.00E+00 0.00E+00 0.00E+00
Module D 4.76E-02 0.00E+00 0.00E+00 -3.20E-01
LEGEND:
Product stage
End-of-life stage
Benefits and loads beyond the system boundary
MS = use of secondary material; CSR = use of renewable secondary fuels; CSNR = use of non-renewable secondary fuels.
Values expressed per declared unit (1 t of ISAC).
DAPHabitat System 11
2.5. Other environmental information describing different waste categories
Hazardous waste disposed Non-hazardous waste disposed Radioactive waste disposed
Unit kg kg kg
Module A1-A3 4.94E-02 4.07E-02 0.00E+00
Module C2 0.00E+00 0.00E+00 0.00E+00
Module C3 0.00E+00 0.00E+00 0.00E+00
Module C4 0.00E+00 0.00E+00 0.00E+00
Module D 7.89E-07 1.42E-03 8.76E-06
LEGENDA:
Product stage
End-of-life stage
Benefits and loads beyond the system boundary
Values expressed per declared unit (1 t of ISAC).
2.6. Environmental information describing output flows
Materials for energy
Components for re-use Materials for recycling Exported energy
recovery
Unidade kg kg kg MJ
Module A1-A3 3.75E-02 8.93E+00 0.00E+00 0.00E+00
Module C2 0.00E+00 0.00E+00 0.00E+00 0.00E+00
Module C3 0.00E+00 1.00E+03 0.00E+00 0.00E+00
Module C4 0.00E+00 0.00E+00 0.00E+00 0.00E+00
Module D 1.00E+03 1.68E-03 8.31E-06 0.00E+00
LEGENDA:
Product stage
End-of-life stage
Benefits and loads beyond the system boundary
Values expressed per declared unit (1 t of ISAC).
2.7. Information describing the biogenic carbon content at the factory gate
Biogenic carbon content Units Modules A1-A3 (results)
Biogenic carbon content in product kg C Not applicable
Biogenic carbon content in accompanying packaging kg C Not applicable
DAPHabitat System 12
3. SCENARIOS AND ADDITIONAL TECHNICAL INFORMATION
3.1. C2 Transport – End-of-life of the product
Results expressed per
Parameter Units
declared unit
Distance km 0
3.2. C3 Waste processing for reuse. recovery and/or recycling – End-of-life of the product
Results expressed per
Parameter Units
declared unit
Material for reuse kg 1,000
3.3. C4 Disposal – End-of-life of the product
Results expressed per
Parameter Units
declared unit
Material for final deposition kg 0
3.4. Scenario and technical information for module D
Results expressed per declared unit
Parameter Units
Reuse of ISAC Recycling of ferrous metals
Net output flow kg 1,000 0.048
Avoided production of gravel kg 1,000 -
Avoided production of steel kg - 0.042
Location of end-of-waste point - In the place of reuse. In the place of recycling.
Steel manufactured from scrap is
ISAC is assumed to have the same considered to have the same quality as
Point of functional equivalence -
quality as gravel. steel manufactured from primary
material.
The net output flow of ferrous metals is
equal to the difference between the
flow of ferrous metals that will be
Assumptions - -
recycled and the input flow of ferrous
metals of secondary origin consumed in
ISAC production.
3.5. Additional information on release of dangerous substances to indoor air, soil, and
water during the use stage
Not applicable.
DAPHabitat System 13
4. REFERENCES
✓ General Instructions of the DAPHabitat System. Version 2.1. Edition August 2023 (in www.daphabitat.pt);
✓ PCR – basic module for construction products and services. DAPHabitat System. Version 2.3. August 2023 (in
www.daphabitat.pt);
✓ ISO 14025:2009 Environmental declarations and labels – Type III environmental declarations – Principles and
procedures;
✓ EN 15804:2012 + A2:2019 Sustainability of construction works – Environmental product declarations – Core
rules for the product category of construction products;
✓ EN 15942:2021 Sustainability of construction works – Environmental product declarations – Communication
format business-to-business.
DAPHabitat System 14
