Environmental product declaration
In accordance with 14025 and EN15804+A2
JACKOPOR VEIBLOKK 5% EPS
Owner of the declaration: Program operator:
Bewi Insulation Scandinavia The Norwegian EPD Foundation
Product: Declaration number:
JACKOPOR VEIBLOKK 5% EPS
Registration number:
Declared unit:
1 m3 Issue date:
This declaration is based on Product Category Rules: Valid to:
CEN Standard EN 15804:2012+A2:2019 serves as core
EPD Software:
PCR
The Norwegian EPD Foundation LCA.no EPD generator ID: 58215
NPCR 012:2022 Part B for thermal insulation products
1 / 11
General information
Product Owner of the declaration:
JACKOPOR VEIBLOKK 5% EPS Bewi Insulation Scandinavia
Contact person: Svein Tore Larsen
Phone: +47 95 07 67 42
e-mail: svein.tore.larsen@jackon.no
Program operator: Manufacturer:
Post Box 5250 Majorstuen, 0303 Oslo, Norway Bewi Insulation Scandinavia
The Norwegian EPD Foundation Sørkilen 3
Phone: +47 23 08 80 00 1621 GRESSVIK, Fredrikstad i VIKEN, Norway
web: post@epd-norge.no
Declaration number: Place of production:
Bewi Insulation Scandinavia, Fredrikstad
Sørkilen 3
NO-1621 Gressvik, Norway
This declaration is based on Product Category Rules: Management system:
CEN Standard EN 15804:2012+A2:2019 serves as core PCR ISO 9001: 185977-2015-AQ-NOR-NA and ISO 14001: 251411-
NPCR 012:2022 Part B for thermal insulation products 2017-AE-NOR-NA
Statement of liability: Organisation no:
The owner of the declaration shall be liable for the underlying 913019334
information and evidence. EPD Norway shall not be liable with respect
to manufacturer information, life cycle assessment data and
evidences.​
Declared unit: Issue date:
1 m3 JACKOPOR VEIBLOKK 5% EPS
Declared unit with option: Valid to:
A1,A2,A3,A4,A5,C1,C2,C3,C4,D
Year of study:
2021
Declared unit, specification: Comparability:
1 m3 Jackopor 100 EPS geofoam for landfill, under roads etc incl EPD of construction products may not be comparable if they not
transportation to site, waste handling and recovery. comply with EN 15804 and seen in a building context.
General information on verification of EPD from EPD tools: Development and verification of EPD:
Independent verification of data, other environmental information The declaration is created using EPD tool lca.tools ver EPD2022.03,
and the declaration according to ISO 14025:2010, § 8.1.3 and § 8.1.4. developed by LCA.no. The EPD tool is integrated in the company's
Individualthird party verification of each EPD is not required when the management system, and has been approved by EPD Norway.
EPD tool is i) integrated into the company's environmental
management system, ii) the procedures for use of the EPD tool are Developer of EPD: Svein Tore Larsen
approved by EPDNorway, and iii)the proccess is reviewed annualy. See
Reviewer of company-specific input data and EPD:​ Jostein Häckert
Appendix G of EPD-Norway's General Programme Instructions for
further information on EPD tools.
Verification of EPD tool: Approved:
Independent third party verification of the EPD tool, background data
and test-EPD in accordance with EPDNorway's procedures and
guidelines for verification and approval of EPD tools.
Third party verifier:
Elisabet Amat
(no signature required)
2 / 11
Product
Product description:
No variation between sites; single production site declared.
Product description
Jackopor Veiblokk 5% is made of expanded polystyrene (EPS) and can be used a geofoam for landfill under roads, bridges, railways. Because of the
low weight and high compressive strength the block are used to minimize the pressure of the construction over the geofoam down to the masses
below.
This product is tested for 5% compressive strength.
Product specification
EPS is manufactured through permeating polystyrene beads with pentane, allowing the beads to expand when exposed to steam. This addition of
a so-called blowing agent adds 4% - 6% w/w.
The expanded polystyrene (EPS) beads are then fed into a block molding machine, where steam and pressure forms large blocks of EPS. The
amount of EPS going into the mold determines the densitiy of the block, where pressure class 100 provides a density at 100 kN/m2, which is
approximately 20 kg/m3. After molding, the remaining blowing agent, pentane, is aired out and the blocks are cut into the desired shape.
Weight per declared unit is 20 kg
Materials kg %
Plastic - Polystyrene expandable (EPS) 20,00 100,00
Total 20,00
Packaging kg %
Packaging - Plastic 0,42 100,00
Total incl. packaging 20,42
Technical data:
CE marking: EPS insulation boards are CE certified according to NS-EN 13163
Compressive strength CS(5): 100 kPa
Typical size: 600 mm x 1200 mm, 1200 x 2400mm
Typical thickness: 400 mm - 1200 mm
Moisture absorption: <5 vol%
Market:
Norway
Reference service life, product
As in the construction where it is used
Reference service life, building or construction works
As in the construction where it is used
LCA: Calculation rules
Declared unit:
1 m3 JACKOPOR VEIBLOKK 5% EPS
Cut-off criteria:
All major raw materials and all the essential energy is included. The production processes for raw materials and energy flows with very small
amounts (less than 1%) are not included. These cut-off criteria do not​ apply for hazardous materials and substances.
Allocation:
The allocation is made in accordance with the provisions of EN 15804. Incoming energy and water and waste production in-house is allocated
equally among all products through mass allocation. Effects of primary production of recycled materials is allocated to the main product in which
the material was used. The recycling process and transportation of the material is allocated to this analysis.
Data quality:
Specific data for the product composition are provided by the manufacturer. The data represent the production of the declared product and were
collected for EPD development in the year of study. Background data is based on EPDs according to EN 15804 and different LCA databases. The
data quality of the raw materials in A1 is presented in the table below.
Materials Source Data quality Year
Packaging - Plastic ecoinvent 3.6 Database 2019
European
Plastic - Polystyrene expandable (EPS) Plastics Europe + ecoinvent 3.6 2019
average.
3 / 11
System boundaries (X=included, MND=module not declared, MNR=module not relevant)
Construction Beyond the system
Product stage Use stage End of life stage
installation stage boundaries
A1 A2 A3 A4 A5 B1 B2 B3 B4 B5 B6 B7 C1 C2 C3 C4 D
X X X X X MND MND MND MND MND MND MND X X X X X
System boundary:
Additional technical information:
waR slairetam tropsnarT gnirutcafunaM tropsnarT ylbmessA e​sU ecnanetniaM riapeR tnemecalpeR tnemhsibrufeR lanoitarepO ygrene esu lanoitarepO esu retaw -eD noitcurtsnoc noitilomed tropsnarT etsaW gnissecorp lasopsiD -yrevoceR-esueR laitnetop-gnilcyceR
4 / 11
LCA: Scenarios and additional technical information
The following information describe the scenarios in the different modules of the EPD.
Capacity utilisation Value
Transport from production place to user (A4) Distance (km) Fuel/Energy Consumption Unit
(incl. return) % (Liter/tonne)
Truck, 16-32 tonnes, EURO 6 (kgkm) 36,7 % 150 0,043 l/tkm 6,45
Assembly (A5) Unit Value
Waste, packaging, plastic to average treatment -
kg 0,42
A5 (inkl transport) (kg)
De-construction demolition (C1) Unit Value
Manual demolition of EPS in C1 kg/DU 20,00
Capacity utilisation Value
Transport to waste processing (C2) Distance (km) Fuel/Energy Consumption Unit
(incl. return) % (Liter/tonne)
Truck, over 32 tonnes, EURO 6 (kgkm) - RER 53,3 % 83 0,023 l/tkm 1,91
Waste processing (C3) Unit Value
Waste, Polystyrene, incineration kg 20,00
Disposal (C4) Unit Value
Landfilling of ashes from incineration of PS kg 0,06
Benefits and loads beyond the system
Unit Value
boundaries (D)
substitution of electricity, Norway MJ 11,60
Substitution of thermal energy, Norway (MJ) MJ 638,64
5 / 11
LCA: Results
The LCA results are presented below for the declared unit defined on page 2 of the EPD document.
Environmental impact
Indicator Unit A1 A2 A3 A4 A5 C1 C2 C3 C4 D
GWP-total
kg CO2 -
4,69E+01 1,54E+00 1,23E+01 4,90E-01 3,36E-02 0,00E+00 1,45E-01 6,38E+01 3,11E-03 -3,63E+00
eq
GWP-fossil
kg CO2 -
4,67E+01 1,54E+00 1,22E+01 4,90E-01 3,36E-02 0,00E+00 1,45E-01 6,38E+01 3,11E-03 -3,50E+00
eq
GWP-biogenic
kg CO2 -
1,95E-01 6,58E-04 6,37E-02 2,03E-04 4,64E-06 0,00E+00 6,19E-05 4,40E-04 1,65E-06 -2,10E-03
eq
GWP-luluc
kg CO2 -
1,14E-02 4,76E-04 2,08E-03 1,74E-04 2,58E-06 0,00E+00 4,40E-05 6,97E-05 4,76E-07 -1,27E-01
eq
kg
ODP CFC11 - 4,14E-08 3,71E-07 2,35E-06 1,11E-07 2,02E-09 0,00E+00 3,49E-08 4,57E-08 3,33E-10 -2,70E-01
eq
mol H+
AP 8,40E-02 5,52E-03 3,61E-02 1,41E-03 4,14E-05 0,00E+00 4,66E-04 7,58E-03 1,09E-05 -2,89E-02
-eq
EP-FreshWater kg P -eq 2,08E-04 1,22E-05 6,38E-05 3,92E-06 6,91E-08 0,00E+00 1,15E-06 4,51E-06 4,20E-08 -3,15E-04
EP-Marine kg N -eq 2,22E-02 1,23E-03 9,03E-03 2,79E-04 3,79E-05 0,00E+00 1,02E-04 3,65E-03 3,41E-06 -9,80E-03
mol N -
EP-Terrestial 2,41E-01 1,37E-02 9,87E-02 3,12E-03 1,48E-04 0,00E+00 1,14E-03 3,90E-02 3,89E-05 -1,06E-01
eq
kg
POCP NMVOC 1,06E-01 5,15E-03 2,95E-01 1,19E-03 4,88E-05 0,00E+00 4,47E-04 9,36E-03 1,07E-05 -2,91E-02
-eq
ADP- kg Sb -
2,31E-05 2,73E-05 2,72E-05 1,35E-05 1,79E-07 0,00E+00 2,58E-06 1,97E-06 1,74E-08 -2,19E-05
minerals&metals1 eq
ADP-fossil1 MJ 1,59E+03 2,50E+01 1,57E+02 7,41E+00 1,38E-01 0,00E+00 2,35E+00 3,91E+00 2,83E-02 -5,02E+01
WDP1 m3 5,68E+01 1,90E+01 6,30E+02 7,17E+00 4,89E-01 0,00E+00 1,80E+00 8,67E+00 2,93E-01 -1,82E+02
GWP total Global Warming Potential total; GWP fossil Global Warming Potential fossil fuels ; GWP biogenic Global Warming Potential biogenic; GWP luluc Global W
Potential land use change; ODP Ozone Depletion; AP Acidification; EP freshwater Eutrophication aquatic freshwater; EP marine Eutrophication aquatic marine; EP
terrestrial Eutrophication terrestrial ;POCP Photochemical zone formation; ADPE Abiotic Depletion Potential minerals and metals; ADPf Abiotic Depletion Potential fossil
fuels;
"Reading example: 9,0 E-03 = 9,0*10-3 = 0,009"
*INA Indicator Not Assessed
1. The results of this environmental impact indicator shall be used with care as the uncertainties on these results are high or as there is limited experienced with the
indicator
Remarks to environmental impacts
6 / 11
Additional environmental impact indicators
Indicator Unit A1 A2 A3 A4 A5 C1 C2 C3 C4 D
PM Disease incidence 6,55E-07 1,41E-07 4,04E-07 3,00E-08 7,45E-10 0,00E+00 1,33E-08 3,19E-08 1,36E-10 -1,84E-06
IRP2 kgBq U235 -eq 1,01E+00 1,09E-01 6,95E-01 3,24E-02 6,26E-04 0,00E+00 1,03E-02 6,53E-03 1,34E-04 -2,89E-01
ETP-fw1 CTUe 7,53E+03 1,82E+01 9,68E+01 5,49E+00 1,32E-01 0,00E+00 1,72E+00 9,42E+00 5,19E-02 -2,76E+02
HTP-c1 CTUh 1,82E-08 0,00E+00 4,15E-09 0,00E+00 3,00E-12 0,00E+00 0,00E+00 2,68E-09 3,00E-12 -4,69E-09
HTP-nc1 CTUh 8,08E-07 1,77E-08 1,25E-07 6,00E-09 1,25E-10 0,00E+00 1,66E-09 1,06E-07 9,60E-11 -2,62E-07
SQP1 dimensionless 4,93E+01 2,84E+01 2,23E+01 5,18E+00 2,42E-01 0,00E+00 2,69E+00 4,65E-01 7,80E-02 -3,53E+02
PM Particulate Matter emissions; IRP Ionizing radiation – human health; ETP-fw Eco toxicity – freshwater; HTP-c Human toxicity – cancer effects; HTP-nc Human
toxicity – non cancer effects; SQP Soil Quality (dimensionless)
"Reading example: 9,0 E-03 = 9,0*10-3 = 0,009"
*INA Indicator Not Assessed
1. The results of this environmental impact indicator shall be used with care as the uncertainties on these results are high or as there is limited experienced with the
indicator
2. This impact category deals mainly with the eventual impact of low dose ionizing radiation on human health of the nuclear fuel cycle. It does not consider effects due
to possible nuclear accidents, occupational exposure nor due to radioactive waste disposal in underground facilities. Potential ionizing radiation from the soil, from
radon and from some construction materials is also not measured by this indicator.
7 / 11
Resource use
Indicator Unit A1 A2 A3 A4 A5 C1 C2 C3 C4 D
PERE MJ 1,02E+01 3,13E-01 4,46E+01 1,06E-01 3,50E-03 0,00E+00 2,95E-02 1,12E-01 1,65E-03 -2,92E+02
PERM MJ 0,00E+00 0,00E+00 0,00E+00 0,00E+00 0,00E+00 0,00E+00 0,00E+00 0,00E+00 0,00E+00 0,00E+00
PERT MJ 1,02E+01 3,13E-01 4,46E+01 1,06E-01 3,50E-03 0,00E+00 2,95E-02 1,12E-01 1,65E-03 -2,92E+02
PENRE MJ 1,03E+03 2,50E+01 1,57E+02 7,41E+00 1,38E-01 0,00E+00 2,35E+00 3,91E+00 2,83E-02 -5,02E+01
PENRM MJ 6,62E+02 0,00E+00 0,00E+00 0,00E+00 0,00E+00 0,00E+00 0,00E+00 0,00E+00 0,00E+00 0,00E+00
PENRT MJ 1,69E+03 2,50E+01 1,57E+02 7,41E+00 1,38E-01 0,00E+00 2,35E+00 3,91E+00 2,83E-02 -5,02E+01
SM kg 6,87E-03 0,00E+00 8,29E-02 0,00E+00 6,61E-05 0,00E+00 0,00E+00 0,00E+00 0,00E+00 0,00E+00
RSF MJ 1,53E-01 1,09E-02 6,16E-02 3,79E-03 9,17E-05 0,00E+00 1,03E-03 3,14E-03 4,10E-05 -2,94E-02
NRSF MJ 1,05E-02 3,60E-02 4,24E-01 1,36E-02 2,40E-04 0,00E+00 3,46E-03 0,00E+00 6,52E-03 -1,93E+01
FW m3 1,32E+00 2,83E-03 4,06E-01 7,92E-04 7,32E-05 0,00E+00 2,67E-04 1,11E-02 2,60E-05 -1,29E-01
PERE Use of renewable primary energy excluding renewable primary energy resources used as raw materials; PERM Use of renewable primary energy resources used as
raw materials; PERT Total use of renewable primary energy resources; PENRE Use of non renewable primary energy excluding non-renewable primary energy resources
used as raw materials; PENRM Use of non renewable primary energy resources used as raw materials; PENRT Total use of non renewable primary energy resources; SM
Use of secondary materials; RSF Use of renewable secondary fuels; NRSF Use of non renewable secondary fuels; FW Use of net fresh water
"Reading example: 9,0 E-03 = 9,0*10-3 = 0,009"
*INA Indicator Not Assessed
8 / 11
End of life - Waste
Indicator Unit A1 A2 A3 A4 A5 C1 C2 C3 C4 D
HWD kg 6,53E-02 1,36E-03 1,07E-01 3,82E-04 5,47E-05 0,00E+00 1,28E-04 0,00E+00 5,16E-02 -7,31E-04
NHWD kg 1,03E+00 2,15E+00 6,38E-01 3,60E-01 2,10E-01 0,00E+00 2,04E-01 0,00E+00 2,55E-02 -1,04E+00
RWD kg 4,84E-05 1,71E-04 1,05E-03 5,05E-05 9,31E-07 0,00E+00 1,60E-05 0,00E+00 1,70E-07 -2,53E-04
HWD = Hazardous waste disposed; NHWD = Non-hazardous waste disposed; RWD = Radioactive waste disposed;
"Reading example: 9,0 E-03 = 9,0*10-3 = 0,009"
*INA Indicator Not Assessed
End of life - Output flow
Indicator Unit A1 A2 A3 A4 A5 C1 C2 C3 C4 D
CRU kg 0,00E+00 0,00E+00 0,00E+00 0,00E+00 0,00E+00 0,00E+00 0,00E+00 0,00E+00 0,00E+00 0,00E+00
MFR kg 2,25E-03 0,00E+00 4,27E-01 0,00E+00 2,16E-01 0,00E+00 0,00E+00 0,00E+00 0,00E+00 0,00E+00
MER kg 5,35E-04 0,00E+00 2,60E-04 0,00E+00 9,66E-07 0,00E+00 0,00E+00 2,00E+01 0,00E+00 0,00E+00
EEE MJ 1,01E-02 0,00E+00 3,35E-01 0,00E+00 2,67E-03 0,00E+00 0,00E+00 3,52E+01 0,00E+00 0,00E+00
EET MJ 1,53E-01 0,00E+00 5,07E+00 0,00E+00 4,04E-02 0,00E+00 0,00E+00 5,33E+02 0,00E+00 0,00E+00
CRU = Components for re-use; MFR = Materials for recycling; MER = Materials for energy recovery; EEE = Exported electrical energy; EET = Exported energy ​ Thermal
"Reading example: 9,0 E-03 = 9,0*10-3 = 0,009"
*INA Indicator Not Assessed
Biogenic Carbon Content
Indicator Unit At the factory gate
Biogenic carbon content in product kg C 0,00E+00
Biogenic carbon content in accompanying packaging kg C 0,00E+00
Note: 1 kg biogenic carbon is equivalent to 44/12 kg CO2
9 / 11
Additional Norwegian requirements
Greenhouse gas emissions from the use of electricity in the manufacturing phase
National production mix from import, low voltage (production of transmission lines, in addition to direct emissions and losses in grid) of applied
electricity for the manufacturing process (A3).
Electricity mix Data source Amount Unit
Electricity, Norway (kWh) ecoinvent 3.6 21,18 g CO2-eq/kWh
Dangerous substances
The product contains no substances given by the REACH Candidate list or the Norwegian priority list.
Indoor environment
Additional Environmental Information
Environmental impact indicators EN 15804+A1 and NPCR Part A v2.0
Indicator Unit A1 A2 A3 A4 A5 C1 C2 C3 C4 D
GWP kg CO2 -eq 1,22E+00 1,53E+00 1,21E+01 4,85E-01 2,76E-02 0,00E+00 1,43E-01 6,38E+01 3,23E-03 -3,57E+00
ODP kg CFC11 -eq 4,28E-08 3,01E-07 1,88E-06 9,00E-08 1,62E-09 0,00E+00 2,82E-08 4,11E-08 2,73E-10 -3,71E-07
POCP kg C2H4 -eq 6,39E-04 1,99E-04 2,64E-01 5,92E-05 4,23E-06 0,00E+00 1,77E-05 8,28E-05 3,69E-07 -4,39E-03
AP kg SO2 -eq 4,54E-03 3,66E-03 2,79E-02 9,68E-04 1,78E-05 0,00E+00 3,01E-04 5,24E-03 5,71E-06 -2,13E-02
EP kg PO43- -eq 4,90E-04 3,98E-04 3,95E-03 1,03E-04 1,34E-05 0,00E+00 3,27E-05 1,70E-03 7,75E-07 -6,34E-03
ADPM kg Sb -eq 1,22E-05 2,73E-05 2,72E-05 1,35E-05 1,79E-07 0,00E+00 2,58E-06 1,97E-06 1,74E-08 -2,19E-05
ADPE MJ 3,34E+01 2,45E+01 1,57E+02 7,26E+00 1,34E-01 0,00E+00 2,30E+00 3,91E+00 2,83E-02 -4,14E+01
GWPIOBC kg CO2 -eq 1,30E+00 1,54E+00 1,18E+01 4,90E-01 0,00E+00 0,00E+00 1,45E-01 6,38E+01 3,23E-03 -3,58E+00
GWP Global warming potential; ODP Depletion potential of the stratospheric ozone layer; POCP Formation potential of tropospheric photochemical oxidants; AP
Acidification potential of land and water; EP Eutrophication potential; ADPM Abiotic depletion potential for non fossil resources; ADPE Abiotic depletion​ potential for
fossil resources; GWP-IOBC/GHG Global warming potential calculated according to the principle of instantanious oxidation (except emissions and uptake of biogenic
carbon)
10 / 11
Bibliography
ISO 14025:2010 Environmental labels and declarations - Type III environmental declarations - Principles and procedures.
ISO 14044:2006 Environmental management - Life cycle assessment - Requirements and guidelines.
EN 15804:2012+A2:2019 Environmental product declaration - Core rules for the product category of construction products.
ISO 21930:2017 Sustainability in buildings and civil engineering works - Core rules for environmental product declarations of construction
products.
ecoinvent v3, Allocation, cut-off by classification, Swiss Centre of Life Cycle Inventories.
Iversen et al., (2021) eEPD v2021.09 Background information for EPD generator tool system verification, LCA.no Report number: 07.21
Vold, M. et al (2022): EPD generator for NPCR 012, Additional products, EPS and XPS, Background information for EPD generator application
NPCR Part A: Construction products and services. Ver. 2.0. April 2021, EPD-Norge.
NPCR 012 Part B for Thermal insulation products, version 2, 31.03.2022, 2022., EPD Norway.
Program operator and publisher Phone: +47 23 08 80 00
The Norwegian EPD Foundation e-mail: post@epd-norge.no
Post Box 5250 Majorstuen, 0303 Oslo, Norway web: www.epd-norge.no
Owner of the declaration: Phone: +47 95 07 67 42
Bewi Insulation Scandinavia e-mail: svein.tore.larsen@jackon.no
Sørkilen 3, 1621 GRESSVIK, Fredrikstad i VIKEN web: www.jackon.no
Author of the Life Cycle Assessment Phone: +47 916 50 916
LCA.no AS e-mail: post@lca.no
Dokka 6B, 1671 web: www.lca.no
Developer of EPD generator Phone: +47 916 50 916
LCA.no AS e-mail: post@lca.no
Dokka 6B,1671 Kråkerøy web: www.lca.no
ECO Platform web: www.eco-platform.org
ECO Portal web: ECO Portal
11 / 11
