ENVIRONMENTAL PRODUCT DECLARATION
as per ISO 14025 and EN 15804+A2
Owner of the Declaration JANSEN AG
Publisher Institut Bauen und Umwelt e.V. (IBU)
Programme holder Institut Bauen und Umwelt e.V. (IBU)
Declaration number EPD-JAN-20230114-CBA1-EN
Issue date 20.10.2023
Valid to 19.10.2028
JANSEN VISS façade width x height: 2500mm x 3200mm
Jansen AG
www.ibu-epd.com | https://epd-online.com
General Information
Jansen AG JANSEN VISS façade width x height: 2500mm x
3200mm
Programme holder Owner of the declaration
IBU – Institut Bauen und Umwelt e.V. JANSEN AG
Hegelplatz 1 Industriestrasse 34
10117 Berlin 9463 Oberriet
Germany Switzerland
Declaration number Declared product / declared unit
EPD-JAN-20230114-CBA1-EN 1 m2 JANSEN VISS façade with a grammage of 45.55 kg/m². The actual
reference size of the declared façade element has dimensions of 2500mm
x 3200mm.
This declaration is based on the product category rules: Scope:
Curtain walling, 01.08.2021 The environmental product declaration refers to a façade type Jansen
(PCR checked and approved by the SVR) VISS in specific dimension width x height. The characteristic values used
for the system components of the JANSEN VISS façade in the LCA are
provided by Jansen AG.
Issue date
The declared product with the dimension 2500mm x 3200mm is defined
20.10.2023
according to the profile series and product characteristics.
The location of the production site is Oberriet/Switzerland.
Valid to
This EPD was created with the help of a semi-automated LCA-Tool.
19.10.2028 The owner of the declaration shall be liable for the underlying information
and evidence; the IBU shall not be liable with respect to manufacturer
information, life cycle assessment data and evidences.
The EPD was created according to the specifications of EN 15804+A2. In
the following, the standard will be simplified as EN 15804.
Verification
The standard EN 15804 serves as the core PCR
Independent verification of the declaration and data according to ISO
14025:2011
Dipl.-Ing. Hans Peters internally X externally
(Chairman of Institut Bauen und Umwelt e.V.)
Florian Pronold Matthias Klingler,
(Managing Director Institut Bauen und Umwelt e.V.) (Independent verifier)
1 Environmental Product Declaration - Jansen AG - JANSEN VISS façade width x height: 2500mm x 3200mm
Product
functions. Our steel façades allow the combination of the
Product description/Product definition visually identical fire protection façade VISS Fire and the
The steel façade system JANSEN VISS can be designed as a burglary- and bullet-resistant VISS RC/FB façade. The VISS
mullion-transom construction or welded as a frame. The Basic add-on construction can be combined with all our VISS
JANSEN VISS façade with face widths of 50 and 60 mm is façades, as well as the structural glazing façade. All Jansen
available with Jansen profiles made of steel in construction window and door systems can be integrated into the Jansen
depths of 18 to 280 mm. Design possible in each case as façade.
burglar-resistant, bullet-resistant, fire-protection façade or SG-
solution, as well as combinations of these properties. The Technical Data
system can also be applied as add-on construction on According to the CE marking, the following structural data for
commercially available beams made of steel, aluminum and the element must be stated:
wood according to static requirements. Our profiles meet
Constructional data
increased thermal insulation requirements with U values from
f Name Value Unit
0.65 W/m²K or 0.51 W/m²K and sound insulation up to 47 dB.
Water tightness acc EN 12154 1200 Pa
Our façade can be planned generally with infill unit weights up
to 1800 kg. Resistance to wind load acc EN 13116 2 kN/m2
Thermal transmittance EN ISO 10077-2 0.65 W/m2K
This declaration describes the following element in JANSEN 47 (-1; -
Sound insulation EN ISO 717-1 dB
VISS: 5)
Product: JANSEN VISS
Air permeability EN 12152 AE class
Face width: 50mm
Impact strength EN 14019 E5 / I5 class
Construction depth: 80mm
Width x height: 2500mm x 3200mm The technical regulations for protecting A category
CE marking according to EN 13830 glazing against falling out TRAV
Further product specifications can be found in the declaration of
For the placing on the market in the European Union/European performance. The properties of the element can be taken from
Free Trade Association (EU/EFTA) the CPR (EU) No. 305/2011/ the CE marking according to EN 13830:2020, curtain wall
applies. The products require a declaration of performance façade. Other constructional data are not relevant for this
taking into account the harmonized product standard EN product.
13830/ curtain walling and a CE marking. The respective
national regulations apply to the use. With this declaration the Base materials/Ancillary materials
following element is declared: JANSEN VISS façade is made of the following materials:
• Glazing approx. 83%
• Steel approx. 12.5%
• Aluminium approx. 2%
• Plastics approx. 2%
• Stainless steel < 1%
The percentages refer to the declared facade with an 8m² area.
The percentages stated may vary depending on the product
type and dimensions.
Does the product or at least one part product contain materials
from the ECHA candidate list of materials which are especially
problematic for approval: Substances of Very High Concern –
SVHC (date 17.01.2023) above a mass percentage of 0.1: no.
This product/article/at least one partial article contains other
carcinogenic, mutagenic, reprotoxic (CMR) substances in
categories 1A or 1B which are not on the candidate list,
exceeding 0.1 percentage by mass: no.
Biocide products were added to this construction product or it
has been treated with biocide products (this then concerns a
treated product as defined by the (EU) Ordinance on Biocide
Products No. 528/2012): no.
Reference service life
According to SBR 2011 regarding the specific material
characteristics of steel, the reference service life is 100 years
(SBR 2011). The practical service life may well be longer.
Conditions for a long service life are regular maintenance, care
Application and upkeep of the product. The specified service life is
independent of the manufacturer's warranty.
The JANSEN VISS façade meets all the requirements of an
interior or exterior wall without taking over load-bearing
2 Environmental Product Declaration - Jansen AG - JANSEN VISS façade width x height: 2500mm x 3200mm
LCA: Calculation rules
EoL stage (modules C1-C4):
Declared Unit Module C1 - considers manual deconstruction (without
The declared unit is 1 m2 of JANSEN VISS façade. environmental burdens).
The actual reference size of the declared façade element has Module C2 - considers 50 km truck transport to waste
dimensions of 2500 mm x 3200 mm. processing. The transport distance can be modified project-
Name Value Unit specific if required by linear scaling.
Declared unit 1 m2 Modules C3 and C4 - consider waste processing and/or
disposal with the following scenarios:
Grammage 45.55 kg/m2
• Scenario 1: 100% thermal treatment of all raw materials
Layer thickness 0.14 m
with heating value including plastic system parts and
For inhomogeneous components made of different materials, 100% recycling of metal system components (C3/1).
the conversion to other dimensions with factors leads to Landfill of all materials without heating value (except
deviations compared to the exact calculation. metals) including glazing (C4/1).
Frame percentage = Frame surface / total area * 100 [%] • Scenario 2 (module C3/2): 100% recycling of plastic
Ground reference = Element depth x element width [m²] system parts and 100% recycling of metal system
components. Landfill of all materials without heating
System boundary
value (except metals) including glazing (C4/2).
Type of EPD according to EN 15804: "cradle to gate with Modules C4/1 & C4/2 are identical.
options, modules C1–C4, and module D". The following
modules are declared: A1–A3, C, D and additional modules: A4 Benefits and loads beyond the product system boundary
+ A5. (module D):
Considers credits and loads from the recycling of the metal
Production (modules A1-A3): components (duplicated in D/1 and D/2) and the recycling of
This module considers the provision of all relevant system the plastic system parts/profiles (D/2). Avoided burdens from
components (i.e. metal profiles/components, glass unit and the thermal treatment of all raw materials with heating value
plastic parts/profiles) and raw materials including their transport (including plastic system parts/profiles) (D/1) and packaging
to the declared production plant. This considers the treatment (duplicated in D/1 and D/2) under European
manufacturing and assembly of these system components, conditions are considered. This affects only the rate of primary
including waste processing up to the end-of-waste state. The materials (no secondary materials).
impact of packaging materials is also covered by this module.
Geographic Representativeness
Transport to the construction site (module A4): Land or region, in which the declared product system is
A distance of 100 km is considered for the transport of the manufactured, used or handled at the end of the product´s
packed finished product via truck. The transport distance can lifespan: Europe
be modified project-specific if required by linear scaling.
Installation (module A5): Comparability
Treatment and disposal of packaging material are considered in Basically, a comparison or an evaluation of EPD data is only
this module. Credits for potential avoided burdens due to possible if all the data sets to be compared were created
energy substitution of electricity and thermal energy generation according to EN 15804 and the building context, respectively
are declared in module D under European conditions and affect the product-specific characteristics of performance, are taken
only the rate of primary materials (no secondary materials). into account.
Electricity consumption for the installation of the declared The following background database has been used for the LCA
product at the construction/building site is also considered. calculation: Sphera LCA software (GaBi ts) content update
package (CUP) version 2022.2
LCA: Scenarios and additional technical information
JANSEN VISS façade.
Characteristic product properties of biogenic carbon
Transport from the gate to the site (A4)
No biogenic carbon is reported in the product. The biogenic
carbon content in the accompanying packaging for 1 m2 Name Value Unit
JANSEN VISS façade is declared below. Litres of fuel 0.0896 l/100km
Transport distance 100 km
Information on describing the biogenic Carbon Content at
factory gate Capacity utilisation (including empty runs) 61 %
Name Value Unit Gross weight of packed products transported 45.56 kg
kg
Biogenic carbon content in product - Assembly (A5)
C
Treatment and disposal of packaging material are considered in
Biogenic carbon content in accompanying kg
0.00327 this module. Electricity consumption for the installation of the
packaging C
declared product at the construction/building site is also
Note: 1 kg of biogenic carbon is equivalent to 44/12 kg of CO considered. The values refer to the declared unit of 1 m2 of
2
JANSEN VISS façade.
The following technical information is a basis for the declared
modules. The values refer to the declared unit of 1 m2 of
3 Environmental Product Declaration - Jansen AG - JANSEN VISS façade width x height: 2500mm x 3200mm
Name Value Unit available in reality due to economic viability limitations
associated with higher costs of sorting smaller shares of
Electricity consumption 7.2 MJ
plastics such as those present in the declared product.
Polyethylene (waste packaging to incineration) 0.000704 kg
Name ValueUnit
Cardboard box (waste packaging to
incineration) 0.00337 kg EoL scenario 1 (modules C3/1 and C4/1)
Wood (waste packaging to incineration) 0.00445 kg Collected separately waste type (façade element) 45.55 kg
Recycling (C3/1) 6.72 kg
According to SBR 2011 regarding the specific material
Energy recovery (C3/1) 0.918 kg
characteristics of steel, the reference service life is 100 years
(SBR 2011). The practical service life may well be longer. Landfilling (C4/1) 37.95 kg
Conditions for a long service life are regular maintenance, care EoL scenario 2 (modules C3/2 and C4/2)
and upkeep of the product. The specified service life is Collected separately (façade element) 45.55 kg
independent of the manufacturer's warranty.
Recycling (C3/2) 7.60 kg
Reference service life Energy recovery (C3/2) 0.038 kg
Name Value Unit Landfilling (C4/2) 37.95 kg
Life Span (according to SBR 2011 100 a
Reuse, recovery and/or recycling potentials (D), relevant
scenario information
End of life (C1-C4)
Module D includes the credits and loads from the recycling of
For the End-of-Life stage two scenarios are considered.
the metal components (duplicated in D/1 and D/2) and the
Scenario 1 considers 100% thermal treatment of all raw
recycling of the plastic system parts/profiles (D/2). Avoided
materials with heating value including plastic system parts and
burdens from the thermal treatment of all raw materials with
100% recycling of metal system components (C3/1). Landfill of
heating value (including plastic system parts/profiles) (D/1) and
all materials without heating value (except metals) including
packaging treatment (duplicated in D/1 and D/2) under
glazing (C4/1). Scenario 2 considers 100% recycling of plastic
European conditions are considered. This affects only the rate
system parts and 100% recycling of metal system components
of primary materials (no secondary materials). A waste
(C3/2). Landfill of all materials without heating value (except
incineration plant with R1-value > 0.6 is assumed.
metals) including glazing (C4/2). Modules C4/1 and C4/2 are
For recycling, a collection rate of 100% is considered.
identical. The recycling of plastics scenario declared in this
EPD is currently considered a scenario that is not widely
4 Environmental Product Declaration - Jansen AG - JANSEN VISS façade width x height: 2500mm x 3200mm
LCA: Results
Results provided in this section are presented relative to 1 m2 of façade type Jansen VISS (reference dimensions 2500 mm x 3200
mm).
For the End-of-Life stage two scenarios are considered:
C3/1 - considers 100% recycling of metal system components (duplicated in D/1 and D/2) and 100% thermal treatment of all raw
materials with heating value including plastic system parts.
C3/2 - considers 100% recycling of metal system components (duplicated in D/1 and D/2) and 100% recycling of plastic system parts.
C4/1 and C4/2 - consider landfill of all materials without heating value (except metals) including glazing. Modules C4/1 and C4/2 are
identical.
D/1 - considers credits and loads from the recycling of the metal components (duplicated in D/1 and D/2). Avoided burdens from
packaging treatment (duplicated in D/1 and D/2) and thermal treatment of all raw materials with heating value (including plastic system
parts/profiles) are considered.
D/2 - considers credits and loads from the recycling of the metal components (duplicated in D/1 and D/2) and the recycling of the
plastic system parts/profiles. Avoided burdens from packaging treatment (duplicated in D/1 and D/2) are considered.
DESCRIPTION OF THE SYSTEM BOUNDARY (X = INCLUDED IN LCA; ND = MODULE OR INDICATOR NOT DECLARED; MNR =
MODULE NOT RELEVANT)
Benefits and
Construction loads beyond
Product stage Use stage End of life stage
process stage the system
boundaries
la ire ta m w a Ry lp p u s tro p s n a rT g n iru tc a fu n a M e h t m o rf tro p s n a rTe tis e h t o t e ta g y lb m e s s A e s U e c n a n e tn ia M ria p e R tn e m e c a lp e R tn e m h s ib ru fe R y g re n e la n o ita re p Oe s u re ta w la n o ita re p Oe s u n o itc u rts n o c -e Dn o itilo m e d tro p s n a rT g n is s e c o rp e ts a W la s o p s iD -e s u e R-y re v o c e R-g n ilc y c e Rla itn e to p
A1 A2 A3 A4 A5 B1 B2 B3 B4 B5 B6 B7 C1 C2 C3 C4 D
X X X X X MND MND MNR MNR MNR MND MND X X X X X
RESULTS OF THE LCA - ENVIRONMENTAL IMPACT according to EN 15804+A2: 1 m2 JANSEN VISS façade (45.55 kg/m2)
Parameter Unit A1-A3 A4 A5 C1 C2 C3/1 C3/2 C4/1 C4/2 D/1 D/2
GWP-total kg CO 2 eq 7.84E+01 2.75E-01 8.4E-01 0 1.38E-01 2.32E+00 2.97E-02 5.69E-01 5.69E-01 -9.65E+00 -9.86E+00
GWP-fossil kg CO 2 eq 7.81E+01 2.72E-01 8.27E-01 0 1.36E-01 2.32E+00 2.97E-02 5.66E-01 5.66E-01 -9.64E+00 -9.85E+00
GWP-
biogenic kg CO 2 eq 2.74E-01 1.15E-03 1.23E-02 0 5.75E-04 9.45E-05 7.53E-06 1.91E-03 1.91E-03 -1.1E-02 -1.24E-02
GWP-luluc kg CO 2 eq 2.3E-02 1.52E-03 5.35E-05 0 7.6E-04 9.73E-06 1.19E-06 1.05E-03 1.05E-03 -8.84E-04 -8.66E-04
kg CFC11
ODP 1.86E-10 1.63E-14 8.15E-12 0 8.17E-15 1.45E-13 1.1E-14 1.33E-12 1.33E-12 -6.53E-12 -2.65E-12
eq
AP mol H+ eq 3.72E-01 2.6E-04 1.21E-03 0 1.3E-04 2.35E-04 7.4E-06 4.02E-03 4.02E-03 -3.26E-02 -3.35E-02
EP-
kg P eq 7.72E-05 8.14E-07 3.71E-07 0 4.07E-07 6.65E-08 8.2E-09 9.6E-07 9.6E-07 -3.44E-06 -1.92E-06
freshwater
EP-marine kg N eq 1.27E-01 8.09E-05 3.32E-04 0 4.04E-05 6.27E-05 2.61E-06 1.03E-03 1.03E-03 -4.38E-03 -4.63E-03
EP-terrestrial mol N eq 1.49E+00 9.72E-04 3.55E-03 0 4.86E-04 1.11E-03 3.58E-05 1.13E-02 1.13E-02 -4.39E-02 -4.66E-02
kg NMVOC
POCP 3.31E-01 2.26E-04 9.38E-04 0 1.13E-04 1.78E-04 7.02E-06 3.12E-03 3.12E-03 -1.54E-02 -1.68E-02
eq
ADPE kg Sb eq 2.61E-04 2.28E-08 9.81E-08 0 1.14E-08 3.61E-09 2.56E-10 5.8E-08 5.8E-08 -1.72E-05 -1.73E-05
ADPF MJ 9.55E+02 3.65E+00 1.75E+01 0 1.82E+00 3.79E-01 2.03E-02 7.42E+00 7.42E+00 -1.07E+02 -1.34E+02
m3 world eq
WDP 3.98E+00 2.45E-03 6.32E-02 0 1.22E-03 2.02E-01 6.04E-03 6.21E-02 6.21E-02 -1.68E+00 -1.77E+00
deprived
GWP = Global warming potential; ODP = Depletion potential of the stratospheric ozone layer; AP = Acidification potential of land and water; EP =
Eutrophication potential; POCP = Formation potential of tropospheric ozone photochemical oxidants; ADPE = Abiotic depletion potential for non-fossil
resources; ADPF = Abiotic depletion potential for fossil resources; WDP = Water (user) deprivation potential)
RESULTS OF THE LCA - INDICATORS TO DESCRIBE RESOURCE USE according to EN 15804+A2: 1 m2 JANSEN VISS façade
(45.55 kg/m2)
Parameter Unit A1-A3 A4 A5 C1 C2 C3/1 C3/2 C4/1 C4/2 D/1 D/2
PERE MJ 1.25E+02 2.07E-01 2.65E+00 0 1.04E-01 9.15E-02 6.66E-03 1.11E+00 1.11E+00 -2.6E+01 -2.34E+01
PERM MJ 1.18E-01 0 -1.18E-01 0 0 0 0 0 0 0 0
PERT MJ 1.25E+02 2.07E-01 2.53E+00 0 1.04E-01 9.15E-02 6.66E-03 1.11E+00 1.11E+00 -2.6E+01 -2.34E+01
PENRE MJ 9.17E+02 3.65E+00 1.75E+01 0 1.83E+00 3.88E+01 3.85E+01 7.43E+00 7.43E+00 -1.08E+02 -1.34E+02
PENRM MJ 3.85E+01 0 -3.24E-02 0 0 -3.85E+01 -3.85E+01 0 0 0 0
PENRT MJ 9.56E+02 3.65E+00 1.75E+01 0 1.83E+00 3.79E-01 2.03E-02 7.43E+00 7.43E+00 -1.08E+02 -1.34E+02
SM kg 3.56E+00 0 0 0 0 0 0 0 0 3.3E+00 3.75E+00
RSF MJ 0 0 0 0 0 0 0 0 0 0 0
NRSF MJ 0 0 0 0 0 0 0 0 0 0 0
FW m3 2.46E-01 2.34E-04 3.87E-03 0 1.17E-04 4.74E-03 1.36E-04 1.88E-03 1.88E-03 -8.86E-02 -8.99E-02
5 Environmental Product Declaration - Jansen AG - JANSEN VISS façade width x height: 2500mm x 3200mm
PERE = Use of renewable primary energy excluding renewable primary energy resources used as raw materials; PERM = Use of renewable primary
energy resources used as raw materials; PERT = Total use of renewable primary energy resources; PENRE = Use of non-renewable primary energy
excluding non-renewable primary energy resources used as raw materials; PENRM = Use of non-renewable primary energy resources used as raw
materials; PENRT = Total use of non-renewable primary energy resources; SM = Use of secondary material; RSF = Use of renewable secondary fuels;
NRSF = Use of non-renewable secondary fuels; FW = Use of net fresh water
RESULTS OF THE LCA – WASTE CATEGORIES AND OUTPUT FLOWS according to EN 15804+A2:
1 m2 JANSEN VISS façade (45.55 kg/m2)
Parameter Unit A1-A3 A4 A5 C1 C2 C3/1 C3/2 C4/1 C4/2 D/1 D/2
HWD kg 1.17E-07 1.75E-11 1.25E-09 0 8.75E-12 3.36E-11 1.32E-12 3.81E-10 3.81E-10 1.08E-08 9.64E-09
NHWD kg 5.47E+00 5.24E-04 3.93E-03 0 2.62E-04 7.19E-02 3.72E-03 3.8E+01 3.8E+01 -4.9E-01 -4.74E-01
RWD kg 1.68E-02 4.5E-06 2.91E-03 0 2.25E-06 2.17E-05 1.43E-06 8.27E-05 8.27E-05 -4.14E-03 -3.37E-03
CRU kg 0 0 0 0 0 0 0 0 0 0 0
MFR kg 2.02E-01 0 0 0 0 6.72E+00 7.6E+00 0 0 0 0
MER kg 0 0 0 0 0 0 0 0 0 0 0
EEE MJ 0 0 1.63E-02 0 0 3.59E+00 3.28E-02 0 0 0 0
EET MJ 0 0 2.93E-02 0 0 6.44E+00 6.84E-02 0 0 0 0
HWD = Hazardous waste disposed; NHWD = Non-hazardous waste disposed; RWD = Radioactive waste disposed; CRU = Components for re-use;
MFR = Materials for recycling; MER = Materials for energy recovery; EEE = Exported electrical energy; EET = Exported thermal energy
RESULTS OF THE LCA – additional impact categories according to EN 15804+A2-optional:
1 m2 JANSEN VISS façade (45.55 kg/m2)
Parameter Unit A1-A3 A4 A5 C1 C2 C3/1 C3/2 C4/1 C4/2 D/1 D/2
Disease
PM 2.56E-06 1.57E-09 1.08E-08 0 7.85E-10 2.28E-09 1.83E-10 4.94E-08 4.94E-08 -3.84E-07 -3.88E-07
incidence
IR kBq U235 eq 2.39E+00 6.59E-04 4.26E-01 0 3.3E-04 3.44E-03 1.71E-04 9.19E-03 9.19E-03 -7.3E-01 -5.98E-01
ETP-fw CTUe 2.31E+03 2.53E+00 5.36E+00 0 1.27E+00 2.09E-01 1.49E-02 4.16E+00 4.16E+00 -2.52E+01 -4.07E+01
HTP-c CTUh 1.39E-07 5.1E-11 9.87E-11 0 2.55E-11 1.43E-11 4.73E-13 6.34E-10 6.34E-10 -4.87E-09 -5.17E-09
HTP-nc CTUh 9.33E-07 2.64E-09 5.02E-09 0 1.32E-09 5.63E-10 1.8E-11 7.02E-08 7.02E-08 -1.2E-07 -1.33E-07
SQP SQP 9.28E+01 1.25E+00 1.61E+00 0 6.27E-01 1.15E-01 7.2E-03 1.54E+00 1.54E+00 -3.42E+00 -1.74E+00
PM = Potential incidence of disease due to PM emissions; IR = Potential Human exposure efficiency relative to U235; ETP-fw = Potential comparative
Toxic Unit for ecosystems; HTP-c = Potential comparative Toxic Unit for humans (cancerogenic); HTP-nc = Potential comparative Toxic Unit for humans
(not cancerogenic); SQP = Potential soil quality index
Disclaimer 1 – for the indicator 'Potential Human exposure efficiency relative to U235'.This impact category deals mainly with the
eventual impact of low dose ionizing radiation on human health of the nuclear fuel cycle. It does not consider effects due to possible
nuclear accidents, occupational exposure or radioactive waste disposal in underground facilities. Potential ionizing radiation from the
soil, from radon and from some construction materials is also not measured by this indicator.
Disclaimer 2 – for the indicators 'abiotic depletion potential for non-fossil resources', 'abiotic depletion potential for fossil resources',
'water (user) deprivation potential, deprivation-weighted water consumption', 'potential comparative toxic unit for ecosystems', 'potential
comparative toxic unit for humans – cancerogenic', 'Potential comparative toxic unit for humans - not cancerogenic', 'potential soil
quality index'. The results of this environmental impact indicator shall be used with care as the uncertainties on these results are high
as there is limited experience with the indicator. This EPD was created using a software tool.
References
Standards requirements and classification
EN 13830 EN 14019
EN 13830: 2020 Curtain walling - Product standard EN 14019:2004,Curtain Walling - Impact resistance -
performance requirements
EN 12154
EN 12154: 2000, Curtain walling - Watertightness - EN 15804
Performance requirements and classification EN 15804:2012+A2:2019+AC:2021, Sustainability of
construction works — Environmental Product Declarations —
EN 13116 Core rules for the product category of construction products
EN 13116: 2001, Curtain walling - Resistance to wind load -
Performance requirements ISO 14025
EN ISO 14025:2011, Environmental labels and declarations —
EN ISO 10077 Type III environmental declarations — Principles and
EN ISO 10077-2: 2017 Thermal performance of windows, doors procedures
and shutters - Calculation of thermal transmittance - Part 2:
Numerical method for frames Further References
EN ISO 717-1 Sphera LCA FE Software (GaBi ts)
EN ISO 717-1: 2020, Acoustics — Rating of sound insulation in Sphera LCA software (GaBi ts) content update package (CUP)
buildings and of building elements — Part 1: Airborne sound version 2022.2 (https://www.gabi-software.com/support/gabi)
insulation
Sphera LCA Calculator Software (GaBi Envision)
EN 12152 GaBi Envision 5.0 Sphera Solution GmbH, the LCA, EPD and
EN 12152: 2002, Curtain walls - Air permeability - Performance Ecodesign tool, http://www.gabi-
6 Environmental Product Declaration - Jansen AG - JANSEN VISS façade width x height: 2500mm x 3200mm
software.com/international/software/gabi-envision/, 2022 www.ibu-epd.com
Jansen LCA tool PCR Part A
LCA tool for façades, windows & door PCR - Part A: Calculation rules for the Life Cycle Assessment
LCA-Tool No.: IBU-JAN-202301-LT1-EN and Requirements on the Background Report, version 1.3,
Developed by Sphera Solutions GmbH Institut Bauen und Umwelt e.V., 2021.
IBU 2021 PCR Part B
Institut Bauen und Umwelt e.V.: General Instructions for the PCR – Part B: Requirements of the EPD for Curtain walling,
EPD programme of Institut Bauen und Umwelt e.V., Version version 1.2, Institut Bauen und Umwelt e.V., www.bau-
2.0, Berlin: Institut Bauen und Umwelt e.V., 2021 umwelt.com, 2022
7 Environmental Product Declaration - Jansen AG - JANSEN VISS façade width x height: 2500mm x 3200mm
Publisher
Institut Bauen und Umwelt e.V. +49 (0)30 3087748- 0
Hegelplatz 1 info@ibu-epd.com
10117 Berlin www.ibu-epd.com
Germany
Programme holder
Institut Bauen und Umwelt e.V. +49 (0)30 3087748- 0
Hegelplatz 1 info@ibu-epd.com
10117 Berlin www.ibu-epd.com
Germany
Author of the Life Cycle Assessment
Sphera Solutions GmbH +49 711 341817-0
Hauptstraße 111- 113 info@sphera.com
70771 Leinfelden-Echterdingen www.sphera.com
Germany
Owner of the Declaration
JANSEN AG 0041717639113
Industriestrasse 34 sustainability@jansen.com
9463 Oberriet www.jansen.com
Switzerland
8 Environmental Product Declaration - Jansen AG - JANSEN VISS façade width x height: 2500mm x 3200mm
