ENVIRONMENTAL PRODUCT DECLARATION
as per ISO 14025 and EN 15804+A2
Owner of the Declaration Ideal Standard International NV
Publisher Institut Bauen und Umwelt e.V. (IBU)
Programme holder Institut Bauen und Umwelt e.V. (IBU)
Declaration number EPD-IDE-20220323-IBB1-EN
Issue date 03.04.2023
Valid to 02.04.2028
Ceramic Toilet set
Ideal Standard International
www.ibu-epd.com | https://epd-online.com
1. General Information
Ideal Standard International Ceramic Toilet set
Programme holder Owner of the declaration
IBU – Institut Bauen und Umwelt e.V. Ideal Standard International NV
Hegelplatz 1 Da Vincilaan 2
10117 Berlin 1935 Zaventem
Germany Belgium
Declaration number Declared product / declared unit
EPD-IDE-20220323-IBB1-EN 1 Toilet set including ceramic bowl, ceramic cistern and tank trim
This declaration is based on the product category rules: Scope:
Toilet set, 01.08.2021 The EPD contains the result for 1 specific Toilet pack produced by Ideal
(PCR checked and approved by the SVR) Standard. The EPD is representative for the production of ceramic bowls
and cisterns in Sevievo (Bulgaria), Armitage (United Kingdom) and Teplice
(Czech Republique), and production of the tank trim in Angouleme
Issue date (France). Note that the results have been separated for the ceramic part
and the tank trim, so the user can easily calculate the results for the Toilet
03.04.2023
pack in which the bowl and the cistern have another weight. The formula is
described further in this document. Foreground data has been provided
directly by Ideal Standard and background LCA data is based on
Valid to
Ecoinvent 3.8 and Industry 2.0 data.
02.04.2028 The owner of the declaration shall be liable for the underlying information
and evidence; the IBU shall not be liable with respect to manufacturer
information, life cycle assessment data and evidences.
The EPD was created according to the specifications of EN 15804+A2. In
the following, the standard will be simplified as EN 15804.
Verification
The standard EN 15804 serves as the core PCR
Independent verification of the declaration and data according to ISO
14025:2011
Dipl.-Ing. Hans Peters internally X externally
(Chairman of Institut Bauen und Umwelt e.V.)
Florian Pronold Vito D'Incognito,
(Managing Director Institut Bauen und Umwelt e.V.) (Independent verifier)
1 Environmental Product Declaration - Ideal Standard International - Ceramic Toilet set
2. Product
2.1 Product description/Product definition The composition of the ceramic:
The product under study is a standard white porcelain toilet
• 100 % ceramic
pack, including the bowl, the cistern and the tank trim (i.e. inlet
The composition of the tank trim :
and outlet valve of the flushing mechanism). The EPD is
representative for all toilet packs produced by Ideal Standard in • +/- 90 % plastics (mainly Acrylonitrile butadiene styrene
Sevlievo (Bulgaria), Armitage (UK) and Teplice (Czech (ABS), but also Polyoxymethylene (POM), polyethene
Republique), in which the ceramic parts are made from vitreous (PE) and polypropylene (PP))
China clay ceramic. The manufacturer can - within the • +/- 10 % steel/brass
framework of the European Regulation N° 305/2011 (CPR) - This product does not contain substances listed in the
present the Declaration of Performance (DOP) of the product candidate list (date: 26.10.2022) exceeding 0.1 percentage by
confirming that the product has a CE marking. mass.
2.2 Application This product does not contain other carcinogenic, mutagenic,
The solution is used in private and public bathrooms. The reprotoxic (CMR) substances in categories 1A or 1B which are
product can be used in new construction and renovation work not on the candidate list, exceeding 0.1 percentage by mass,
for hygienic and household use.
Biocide products were not added to this construction product
2.3 Technical Data and it has not been treated with biocide products as defined by
Constructional data the (EU) Ordinance on Biocide Products No. 528/2012.
Name Value Unit 2.6 Manufacture
Minimum 1 1. Slip preparation
Crazing test Internal test - 1hr in autoclave
cycle without - Production of the ceramic mixture (slip) and unloading/storage
with 5 bar steam
crazing of raw materials in the area.
Water absorption EN997 for WC pans
(toilets) and so by extension to the <0.5 % 2. Glaze preparation
Vitreous China products Production of glaze with needed colour.
Minimum 1
Impact resistance Internal test – Ball
drop without - 3. Casting shop
bearing dropped from fixed height
breaking Casting of ceramic products in different moulds.
Resistance to temperature change EN
4. Dryers
14688 for Wash Basins. 1000 hot (75 No visible
- Drying is the process of taking off the humidity and the final
degC) / cold (15 degC) water cycles damage
results are dried products.
without visible damage
Resistance to chemicals and staining EN
5. White inspection
14688 for Wash Basins therefore by
No remaining The first inspection of dried ceramic products. The main focus
extension to other Ceramic Products.
chemical - is checking the quality and cleaning the surface of the products.
Specific chemicals in contact then cleaned
evident At the end of the process the products are grouped in three
with specific apparatus without permanent
different directions: A grade products, products for repairing and
marking
scrap.
Resistance to abrasion EN 14688 for
Wash Basins therefore by extension to No scratches 6. Spraying
other Ceramic Products. Loaded diamond through outer - Covering the ceramic product with glaze
tool (scratch) / Loaded abrasive paper (glaze) layer
wheel (abrasion) for repeated cycles. 7. Kilns
Load resistance 400 kg Firing of ceramic products
The manufacturer can - within the framework of the European
8. Gloss inspection
Regulation N° 305/2011 (CPR) - present the Declaration of
Final inspection for visual control of all products for visible
Performance (DOP) of the product confirming that the product
defects. Separating the products again in three groups: for
has a CE marking.
packaging, for repairing by hand or for grinding machines and
2.4 Delivery status scrap (pitcher).
The products are packed: wooden pallet, PE plastic foil and
coverage carton, and are accompanied with an instruction and 9. Packaging
guarantee sheet. Different kinds of activities for the packaging of the products.
The products can come in different shapes and dimensions. An *Moulds making
overview of all different toilet packs can be found on Ideal Development of a new matrix for production of gypsum moulds
Standard's website and filter on 'Toilet packs': for casting and repairing of the damaged matrix.
https://www.idealstandard.co.uk/products/catalog/toilets/toilet-
packs *Mould shop
Production of gypsum moulds for casting ceramic products and
2.5 Base materials/Ancillary materials polyurethane setters for supporting the casting process.
The main components of the product are: ceramic bowl,
2.7 Environment and health during manufacturing
ceramic cistern and tank trim.
2 Environmental Product Declaration - Ideal Standard International - Ceramic Toilet set
Environmental, occupational health, safety and quality Fire
management at the Ideal Standard plants are in accordance Not subjected to fire classification
with the following standards: Water
• ISO 14001 No risks are expected to occur in terms of environmental and
• ISO 9001 human health.
• ISO 45001
Mechanical destruction
2.8 Product processing/Installation In case of mechanical destruction, no risks are expected to
It is considered that there is no assembly waste, based on the occur in terms of environment and human health.
fact that the product is prefabricated and installed by hand.
2.14 Re-use phase
2.9 Packaging It is possible to partially recycle ceramic products in the
A wooden pallet, PE plastic bag and coverage carton are used production process. This is already applied for production
to pack and transport the product to the supplier/customer. The waste. The recycling of post-consumer waste depends on the
product is also accompanied with an instruction and guarantee sorting and take-back of these waste streams at the demolition
sheet. site.
2.10 Condition of use 2.15 Disposal
The product will not change in material composition during use. According to the average European end-of-life scenario
described in Annexe C of the Product Environmental Footprint
2.11 Environment and health during use Pilots (PEFCR) 6.3 guidance (version March 2018), the
Under normal conditions of use, the product do not cause any following disposal scenarios have been considered: 100 % of
adverse health effects or release of volatile organic compounds the ceramic is landfilled, 45 % of the plastic parts are
(VOCs) into indoor air. incinerated and 55 % of the plastic parts are landfilled.
No environmental impact on water, air or soil is expected. 2.16 Further information
Additional information on toilet packs produced by Ideal
2.12 Reference service life Standard can be found at:
The reference service life is not included, as module B is not https://www.idealstandard.co.uk/products/catalog/toilets/toilet-
considered. packs
2.13 Extraordinary effects
3. LCA: Calculation rules
• Packaging and transport of ancillary materials used
3.1 Declared Unit during the production process
Declared unit • Packaging and transport of ancillary materials used
during installation
Name Value Unit
No further approximations have been made to replace the
Declared unit 1 pce.
missing data, as they were considered to be not relevant based
Mass per piece set 26.93 kg on the first iterations of the results.
Mass of the bowl 15.76 kg
3.4 Cut-off criteria
Mass of the cistern 10.5 kg
Mass of the tank trim 0.67 kg • Big bags used as packaging of some raw materials for
the ceramic production, as they are reused.
The weight of the bowl and the cistern are based on a specific
• For production waste only most relevant production
toilet pack that has been sold most by Ideal Standard in 2021.
waste streams have been considered (waste of ancillary
The results for toilet packs with other weights can be calculated
materials and smaller waste flows have been excluded).
using the Annexe, in which the results for 1 kg ceramic and 1
• Only most relevant ancillary materials have been
piece Tank trim have been described separately.
selected based on consumption rate and importance in
the production process.
This EPD is calculated using the production data of the factory
• Environmental impacts caused by the personnel of the
in Bulgaria. However, a variability study has been performed to
production plants are not included in the LCA, e.g.
show that the production in Bulgaria is representative for the
waste from the cafeteria and sanitary installations,
production by Ideal Standard in the United Kingdom and the
accidental pollution caused by human mistakes, or
Czech Republique. This is further described in paragraph 3.6.
environmental effects caused by commuter traffic.
Heating or cooling of the plants in order to ensure a
3.2 System boundary
comfortable indoor climate for the personnel for
Cradle-to-gate with options, including module D
example is also neglected.
3.3 Estimates and assumptions
3.5 Background data
The following processes are excluded because data was not
Ecoinvent 3.8 and Industry 2.0
available:
• Packaging of the following raw materials used to 3.6 Data quality
produce the glaze of the ceramic products: barium Foreground data is specific to Ideal Standard and is collected
carbonate, sodium carbonate, sodium silicate, for the reference year 2021. Background data is based on
aluminium hydroxide, aluminium oxide, zinc oxide and Ecoinvent 3.8 which is released in September 2021, and
stains Industry 2.0.
• Transport packaging final product The LCA background report includes a variability study
3 Environmental Product Declaration - Ideal Standard International - Ceramic Toilet set
between the different factory plants, respectively Sevlievo
(Bulgaria), Armitage (United Kingdom) and Teplice (Czech 3.9 Allocation
Republique). The results show that the over the total life cycle EN15804+A2 also describes the rules for joint co-production,
(A1-C4) the variance is <40 %. where the processes cannot be divided. This is, however, not
the case in this study. Allocation of secondary materials or
3.7 Period under review secondary fuels is also not applicable for this study.
The data collected by Ideal Standard is based on data from the
production year 2021 for both the ceramics and the tank trim. 3.10 Comparability
Basically, a comparison or an evaluation of EPD data is only
3.8 Geographic Representativeness possible if all the data sets to be compared were created
Land or region, in which the declared product system is according to EN 15804 and the building context, respectively
manufactured, used or handled at the end of the product´s the product-specific characteristics of performance, are taken
lifespan: Europe into account. Ecoinvent 3.8 and Industry 2.0
4. LCA: Scenarios and additional technical information
End of life (C1-C4)
Characteristic product properties of biogenic carbon
According to the average European end-of-life scenario
The product does not contain biogenic carbon, but its
described in Annexe C of the Product Environmental Footprint
accompanying packaging contains 2.30 kg C per product in the
Pilots (PEFCR) 6.3 guidance (version March 2018), the
form of paper, cardboard and wooden pallets.
following disposal scenarios have been considered: 100 % of
Information on describing the biogenic Carbon Content at the ceramic parts are landfilled, 45 % of the plastic parts are
factory gate incinerated, 55 % of the plastic parts are landfilled, 95 % of the
Name ValueUnit smaller metal parts are recycled and 5 % of the smaller metal
kg parts are landfilled.
Biogenic Carbon Content in product 0
C Name Value Unit
Biogenic Carbon Content in accompanying kg Collected as mixed construction waste 26.93 kg
2.30
packaging C Reuse 0 kg
Landfill of ceramics (from bowl and cistern) 26.26 kg
Landfill of plastics (from tank trim) 0.337 kg
Landfill of metals (from tank trim) 0.003 kg
Transport to the building site (A4) Incineration of plastics (from tank trim) 0.275 kg
Name Value Unit Recycling of metals (from tank trim) 0.05 kg
Litres of fuel 254 l/100km
Reuse, recovery and/or recycling potentials (D), relevant
Transport distance 2000 km
scenario information
Capacity utilisation (including Default value
% Module D contains the benefits and loads of recycling the
empty runs) Ecoinvent
smaller metal parts and the benefits of energy recovery during
Gross density of products
Not calculated kg/m3 the incineration of the plastics.
transported
Name ValueUnit
Default value
Capacity utilisation volume factor - Loads recycling of brass: Impact of the production
Ecoinvent
process of brass excluding the production of raw 0.05 kg
Installation into the building (A5) materials
It is considered that there is no assembly waste, Benefits recycling of brass: Avoided production of
0.05 kg
based on the fact that the product is prefabricated and installed brass using 100 % primary materials
by hand. Benefits energy recovery during incineration of
plastics from tank trim: 20 % avoided production of 1.70 MJ
Only the impact of packaging waste has been considered. Heat from natural gas
Name ValueUnit Benefits energy recovery during incineration of
Packaging waste (paper and cardboard) PEF EOL plastics from tank trim: 10 % avoided production of 0.85 MJ
scenario Europe for coverage carton packaging: 11 1.08 kg European average grid mix
% incineration; 75 % recycling; 14 % landfill
Packaging waste (PE) PEF EOL scenario Europe
for PE packaging: 32 % incineration; 29 % 0.05 kg
recycling; 39 % landfill
Packaging waste (wooden pallet) PEF EOL
scenario Europe for wooden pallets: 32 % 2.91 kg
incineration; 30 % recycling; 38 % landfill
4 Environmental Product Declaration - Ideal Standard International - Ceramic Toilet set
5. LCA: Results
An annexe is added to this EPD in which the environmental impact is presented separately for 1 kg ceramics and 1 piece of tank trim,
allowing the user to calculate the environmental impact of toilet packs that include a bowl and/or a cistern with another weight.
DESCRIPTION OF THE SYSTEM BOUNDARY (X = INCLUDED IN LCA; ND = MODULE OR INDICATOR NOT DECLARED; MNR =
MODULE NOT RELEVANT)
Benefits and
Construction loads beyond
Product stage Use stage End of life stage
process stage the system
boundaries
la ire ta m w a Ry lp p u s tro p s n a rT g n iru tc a fu n a M e h t m o rf tro p s n a rTe tis e h t o t e ta g y lb m e s s A e s U e c n a n e tn ia M ria p e R tn e m e c a lp e R tn e m h s ib ru fe R y g re n e la n o ita re p Oe s u re ta w la n o ita re p Oe s u n o itc u rts n o c -e Dn o itilo m e d tro p s n a rT g n is s e c o rp e ts a W la s o p s iD -e s u e R-y re v o c e R-g n ilc y c e Rla itn e to p
A1 A2 A3 A4 A5 B1 B2 B3 B4 B5 B6 B7 C1 C2 C3 C4 D
X X X X X MND MND MNR MNR MNR MND MND X X X X X
RESULTS OF THE LCA - ENVIRONMENTAL IMPACT according to EN 15804+A2: 1 piece installed toilet set
Parameter Unit A1 A2 A3 A4 A5 C1 C2 C3 C4 D
GWP-total kg CO 2 eq 3.75E+00 3.88E+00 3.28E+01 1.08E+01 9.3E+00 4.03E-03 2.3E-01 7.8E-05 8.72E-01 -5.48E+00
GWP-fossil kg CO 2 eq 3.73E+00 3.88E+00 4.05E+01 1.08E+01 1.29E+00 4E-03 2.3E-01 7.73E-05 8.71E-01 -1.52E+00
GWP-
biogenic kg CO 2 eq 1.13E-02 1.35E-03 -7.79E+00 3.87E-03 8E+00 2.22E-05 8.23E-05 4.19E-07 3.35E-04 -3.95E+00
GWP-luluc kg CO 2 eq 3.27E-03 1.66E-03 2.38E-02 4.33E-03 8.76E-05 9.45E-06 9.2E-05 1.79E-07 1.34E-04 -4.11E-03
ODP kg CFC11 eq 4.07E-07 8.88E-07 4.1E-06 2.51E-06 4.45E-08 2.01E-10 5.33E-08 4.01E-12 6.47E-08 -1.77E-07
AP mol H+ eq 1.95E-02 2.06E-02 1.35E-01 3.07E-02 1.14E-03 2.27E-05 6.53E-04 4.43E-07 1.61E-03 -7.87E-03
EP-
kg P eq 1.98E-04 2.65E-05 3.22E-03 7.72E-05 2.28E-06 4.27E-07 1.64E-06 8.11E-09 5.42E-06 -9.28E-05
freshwater
EP-marine kg N eq 3.05E-03 4.6E-03 2.27E-02 6.11E-03 4.35E-04 2.9E-06 1.3E-04 5.9E-08 6.05E-04 -1.77E-03
EP-terrestrial mol N eq 3.46E-02 5.12E-02 2.28E-01 6.81E-02 4.42E-03 3.34E-05 1.45E-03 6.78E-07 6.21E-03 -1.95E-02
kg NMVOC
POCP 1.06E-02 1.61E-02 6.71E-02 2.62E-02 1.33E-03 9.18E-06 5.56E-04 1.9E-07 1.75E-03 -6.05E-03
eq
ADPE kg Sb eq 4.36E-05 9.97E-06 3.51E-05 2.93E-05 5.34E-07 2.16E-08 6.23E-07 4.38E-10 4.61E-07 -2.02E-05
ADPF MJ 7.35E+01 5.8E+01 7.67E+02 1.64E+02 3.01E+00 8.47E-02 3.49E+00 1.62E-03 4.78E+00 -2.82E+01
m3 world eq
WDP 3.34E+00 1.71E-01 1.32E+01 5E-01 1.79E-02 9.92E-04 1.06E-02 1.9E-05 2.98E-02 -1.57E+00
deprived
GWP = Global warming potential; ODP = Depletion potential of the stratospheric ozone layer; AP = Acidification potential of land and water; EP =
Eutrophication potential; POCP = Formation potential of tropospheric ozone photochemical oxidants; ADPE = Abiotic depletion potential for non-fossil
resources; ADPF = Abiotic depletion potential for fossil resources; WDP = Water (user) deprivation potential)
RESULTS OF THE LCA - INDICATORS TO DESCRIBE RESOURCE USE according to EN 15804+A2: 1 piece installed toilet set
Parameter Unit A1 A2 A3 A4 A5 C1 C2 C3 C4 D
PERE MJ 5.85E+00 7.85E-01 3.47E+01 2.31E+00 1.72E+01 1.68E-02 4.9E-02 3.18E-04 2.52E-01 0
PERM MJ 3.04E-02 0 7.74E+01 0 -5.68E+01 0 0 0 0 3.97E+01
PERT MJ 5.88E+00 7.85E-01 1.12E+02 2.31E+00 -3.96E+01 1.68E-02 4.9E-02 3.18E-04 2.52E-01 3.97E+01
PENRE MJ 6.95E+01 5.83E+01 8.37E+02 1.65E+02 1.78E+01 1.01E-01 3.51E+00 1.92E-03 1.09E+01 0
PENRM MJ 1.35E+01 0 4.6E+01 0 -2.81E+01 0 0 0 -6.04E+00 1.34E+01
PENRT MJ 8.3E+01 5.83E+01 8.83E+02 1.65E+02 -1.03E+01 1.01E-01 3.51E+00 1.92E-03 4.89E+00 1.34E+01
SM kg 2.79E-01 0 0 0 0 0 0 0 0 2.69E+00
RSF MJ 0 0 0 0 0 0 0 0 0 0
NRSF MJ 0 0 0 0 0 0 0 0 0 0
FW m3 1.87E-01 4.1E-03 1.91E-01 1.21E-02 1.47E-03 6.39E-05 2.56E-04 1.21E-06 4.91E-03 -4.1E-02
PERE = Use of renewable primary energy excluding renewable primary energy resources used as raw materials; PERM = Use of renewable primary
energy resources used as raw materials; PERT = Total use of renewable primary energy resources; PENRE = Use of non-renewable primary energy
excluding non-renewable primary energy resources used as raw materials; PENRM = Use of non-renewable primary energy resources used as raw
materials; PENRT = Total use of non-renewable primary energy resources; SM = Use of secondary material; RSF = Use of renewable secondary fuels;
NRSF = Use of non-renewable secondary fuels; FW = Use of net fresh water
RESULTS OF THE LCA – WASTE CATEGORIES AND OUTPUT FLOWS according to EN 15804+A2:
1 piece installed toilet set
Parameter Unit A1 A2 A3 A4 A5 C1 C2 C3 C4 D
HWD kg 9.39E-05 1.45E-04 7.05E-04 4.29E-04 7.32E-06 6.44E-08 9.1E-06 1.33E-09 6.07E-06 -4.1E-05
NHWD kg 1.69E+00 2.83E+00 1.36E+01 8.6E+00 2E+00 3.1E-04 1.83E-01 6.3E-06 2.66E+01 -2.19E-01
RWD kg 2.23E-04 3.93E-04 2.16E-03 1.11E-03 1.9E-05 6.19E-07 2.36E-05 1.18E-08 2.91E-05 -1.09E-04
CRU kg 0 0 0 0 0 0 0 0 0 0
MFR kg 0 0 4.23E-03 0 2.91E+00 0 0 5.13E-02 0 -2.97E+00
MER kg 0 0 0 0 0 0 0 0 0 0
5 Environmental Product Declaration - Ideal Standard International - Ceramic Toilet set
EEE MJ 0 0 1.48E-03 0 3.14E+00 0 0 0 2.83E-01 -3.42E+00
EET MJ 0 0 2.95E-03 0 6.28E+00 0 0 0 5.65E-01 -6.84E+00
HWD = Hazardous waste disposed; NHWD = Non-hazardous waste disposed; RWD = Radioactive waste disposed; CRU = Components for re-use;
MFR = Materials for recycling; MER = Materials for energy recovery; EEE = Exported electrical energy; EET = Exported thermal energy
RESULTS OF THE LCA – additional impact categories according to EN 15804+A2-optional:
1 piece installed toilet set
Parameter Unit A1 A2 A3 A4 A5 C1 C2 C3 C4 D
Disease
PM 1.5E-07 2.96E-07 9.56E-07 8.7E-07 2.01E-08 6.27E-11 1.85E-08 1.48E-12 2.91E-08 -1.39E-07
incidence
IR kBq U235 eq 3.72E-01 2.52E-01 2.51E+00 7.13E-01 1.34E-02 7.51E-04 1.51E-02 1.42E-05 2.43E-02 -1.16E-01
ETP-fw CTUe 8.36E+01 4.49E+01 1.71E+02 1.29E+02 3.29E+00 5.36E-02 2.74E+00 1.07E-03 4.61E+00 -2.48E+01
HTP-c CTUh 4.24E-09 1.56E-09 1.39E-08 4.14E-09 5.65E-10 1.65E-12 8.8E-11 5.4E-14 2.13E-10 -7.79E-10
HTP-nc CTUh 6.79E-08 4.44E-08 3.05E-07 1.3E-07 4.53E-09 5.26E-11 2.77E-09 1.06E-12 2.86E-09 -3.8E-08
SQP SQP 3.69E+01 3.81E+01 5.54E+02 1.14E+02 2.72E+00 1.54E-02 2.43E+00 1.06E-03 8.83E+00 -4.16E+02
PM = Potential incidence of disease due to PM emissions; IR = Potential Human exposure efficiency relative to U235; ETP-fw = Potential comparative
Toxic Unit for ecosystems; HTP-c = Potential comparative Toxic Unit for humans (cancerogenic); HTP-nc = Potential comparative Toxic Unit for humans
(not cancerogenic); SQP = Potential soil quality index
Disclaimer 1 – for the indicator “Potential Human exposure efficiency relative to U235”. This impact category deals mainly with the
eventual impact of low-dose ionizing radiation on human health of the nuclear fuel cycle. It does not consider effects due to possible
nuclear accidents, occupational exposure or radioactive waste disposal in underground facilities. Potential ionizing radiation from the
soil, radon and from some construction materials is also not measured by this indicator.
Disclaimer 2 – for the indicators “abiotic depletion potential for non-fossil resources”, “abiotic depletion potential for fossil resources”,
“water (user) deprivation potential, deprivation-weighted water consumption”, “potential comparative toxic unit for ecosystems”,
“potential comparative toxic unit for humans – cancerogenic”, “Potential comparative toxic unit for humans - not cancerogenic”,
“potential soil quality index”. The results of this environmental impact indicator shall be used with care as the uncertainties on these
results are high as there is limited experience with the indicator.
6. LCA: Interpretation
For the toilet pack, more than 90 % of the impact is related to
the ceramic parts in the case of a total ceramic weight of 26,26
kg. However, note that the contribution of the tank trim will For the tank trim, the raw materials or module A1 has the
increase with decreasing weights of the ceramic parts. largest contribution on all impact categories. The second most
important module, is module A3 or the manufacturing process.
For the ceramic parts, the manufacturing or module A3 (and in Outside the system's boundaries, module D shows the benefits
particular energy consumption) has the largest contribution on from the energy recovery from the incineration of the plastic
all impact categories. Besides the manufacturing, also transport components and to a lesser extent the recycling of the small
to the installation site has a significant contribution, due to the steel components in the tank trim. In module D the use of
weight of the product. The impact of recycled content at the beginning of life has been taken into
the raw materials is less significant. account in the calculations, as required by EN15804+A2.
7. Requisite evidence
8. References
Standards ISO 14001
ISO 14001:2015: Environmental management systems —
EN15804 Requirements with guidance for use
EN 15804:2012+A2:2019+AC:2021, Sustainability of
construction works — Environmental Product Declarations — ISO 14025
Core rules for the product category of construction products. EN ISO 14025:2011, Environmental labels and declarations —
Type III environmental declarations — Principles and
PCR Part A procedures.
Calculation rules for the Life Cycle Assessment and
Requirements on the Background Report, Institut Bauen und ISO 14040
Umwelt e.V., www.bauumwelt.com. ISO 14040:2006: Environmental management – Life cycle
assessment – Principles and framework.
PCR Part B
Institut Bauen und Umwelt e.V, Berlin (pub.): PCR Guidance- ISO 14044
Texts for Building-Related Products and Services From the ISO 14044:2006: Environmental management – Life cycle
range of Environmental Product Declarations of Institute assessment – Requirements and guidelines.
Construction and Environment e.V. (IBU) : Requirements on the
EPD for Toilet set ISO 45001
ISO 45001:2018: Occupational health and safety management
ISO 9001 systems Requirements with guidance for use
ISO 9001:2015: Quality management systems — Requirements
Further references
6 Environmental Product Declaration - Ideal Standard International - Ceramic Toilet set
Industry 2.0
Pré Consultants (2021) Industry 2.0 (from PlasticsEurope, worldsteel and ERASM) LCA
SimaPro 9.3.0.3 [Computer Software]. Amersfoort, The database as integrated in SimaPro 9.3.0.3.
Netherlands.
PEFCR
CPR European commission (2018). Product Environmental Footprint
European Regulation N° 305/2011 (CPR) Category Rules PEFCR Guidance, version 6.3.
Ecoinvent IBU
Wernet, G., Bauer, C., Steubing, B., Reinhard, J., Moreno-Ruiz, IBU 2021. Institut Bauen und Umwelt e.V.: General Instructions
E., and Weidema, B., 2016. The ecoinvent database version 3 for the EPD programme of Institut Bauen und Umwelt e.V.,
(part I): overview and methodology. The International Journal of Version 2.0, Berlin: Institut Bauen und Umwelt e.V., 2021
Life Cycle Assessment, [online] 21(9), pp.1218–1230. Available www.ibu-epd.com
at:http://link.springer.com/10.1007/s11367-016-1087-8
REACH candidate list
EN 997 ECHA, REACH Candidate List of substances of very
WC pans and WC suites with integral trap - constructional and highconcern for Authorisation, 26/10/2022
performance requirements.
Biocide Products No. 528/2012
EN 14688 EU, REGULATION (EU) No 528/2012 OF THE
Sanitary appliances. Wash basins. Functional requirements and EUROPEANPARLIAMENT AND OF THE COUNCIL concerning
test methods the makingavailable on the market and use of biocidal
products, 22 May2012
7 Environmental Product Declaration - Ideal Standard International - Ceramic Toilet set
Publisher
Institut Bauen und Umwelt e.V. +49 (0)30 3087748- 0
Hegelplatz 1 info@ibu-epd.com
10117 Berlin www.ibu-epd.com
Germany
Programme holder
Institut Bauen und Umwelt e.V. +49 (0)30 3087748- 0
Hegelplatz 1 info@ibu-epd.com
10117 Berlin www.ibu-epd.com
Germany
Author of the Life Cycle Assessment
Enperas +32 3 376 00 19
Thorpark 8300 info@enperas.com
3600 Genk https://www.enperas.com/en/
Belgium
Owner of the Declaration
Ideal Standard International NV +32(0)28004800
Da Vincilaan 2 eboukari@idealstandard.com
1935 Zaventem www.idealstandard.com
Belgium
8 Environmental Product Declaration - Ideal Standard International - Ceramic Toilet set
