ENVIRONMENTAL PRODUCT DECLARATION
as per ISO 14025 and EN 15804+A2
Owner of the Declaration Kingspan Insulation B.V.
Programme holder Institut Bauen und Umwelt e.V. (IBU)
Publisher Institut Bauen und Umwelt e.V. (IBU)
Declaration number EPD-KIN-20230016-CBA1-EN
Issue date 07.02.2023
Valid to 06.02.2028
Kingspan Sauna-Satu®
Kingspan Insulation B.V.
www.ibu-epd.com | https://epd-online.com
Umwelt Produktdeklaration Name des Herstellers – Name des Produkts
General Information
Kingspan Insulation B.V. Kingspan Sauna-Satu®
Programme holder Owner of the declaration
IBU – Institut Bauen und Umwelt e.V. Kingspan Insulation Oy
Hegelplatz 1 Sillanpäänkatu 20
10117 Berlin 38710 Kankaanpää
Germany Finland
Declaration number Declared product / declared unit
EPD-KIN-20230016-CBA1-EN Kingspan Sauna-Satu®
1m2, 30mm thickness, R = 1,35 m2.K/W
D
This declaration is based on the product Scope:
category rules: The insulation material Kingspan Sauna-Satu® is
Insulating materials made of foam plastics, 01.2019 produced by Kingspan Insulation at the manufacturing
(PCR checked and approved by the SVR) facility in Kankaanpää (Finland).
Issue date Kingspan Sauna-Satu® is an insulation board with a
07.02.2023 rigid thermoset polyisocyanurate (PIR) fibrefree
insulation core, faced on both sides with a
low emissivity composite foil. Kingspan Sauna-
Valid to
Satu® is used as thermal insulation of sauna walls and
06.02.2028
ceilings.
The owner of the declaration shall be liable for the
underlying information and evidence; the IBU shall not
be liable with respect to manufacturer information, life
cycle assessment data and evidences.
The EPD was created according to the specifications
of EN 15804+A2. In the following, the standard will be
simplified as EN 15804.
Verification
The standard EN 15804 serves as the core PCR
Independent verification of the declaration and data
according to ISO 14025:2011
Dipl. Ing. Hans Peters internally x externally
(chairman of Institut Bauen und Umwelt e.V.)
Dr. Alexander Röder Vito D'Incognito
(Managing Director Institut Bauen und Umwelt e.V.)) (Independent verifier)
Product
Product description/Product definition Application
Kingspan Sauna-Satu® is an insulation board with a Kingspan Sauna-Satu® is used as thermal insulation
rigid thermoset polyisocyanurate (PIR) fibre-free of sauna walls and ceilings.
insulation core, faced on both sides with a
low emissivity composite foil. The product is available Technical Data
in 30 mm thickness. This EPD is based on a thickness
of 30 mm and R -value of 1,35 m²·K/W.
D
Constructional data
For the placing on the market of the product in the Name Value Unit
European Union/European Free Trade Association Thermal conductivity according to
0.022 W(m.K)
(EU/EFTA) (with the exception of Switzerland) EN 13165
Regulation (EU) No. 305/2011 (CPR) applies. The Reaction to fire according to EN
E
product needs a declaration of performance taking into 13165
consideration EN 13165 - Thermal insulation products Compressive strength according CS(10\Y)
for buildings - Factory made polyurethane foam to EN 13165 100
(PU) products - Specification and the CE-marking. For Thickness tolerance according to
T2
the application and use the respective national EN 13165
provisions apply.
2 Environmental Product Declaration Kingspan Insulation B.V. – Kingspan Sauna-Satu®
Performance data of the product in accordance with exempt from the requirements of Articles 57 and 59(1)
the declaration of performance with respect to its of REACH Regulation (EC) No 1907/2006. These
essential characteristics according to EN 13165 - products are not classified as “hazardous products”
Thermal insulation products for buildings - Factory according to any current legislation, and can hence be
made rigid polyurethane foam (PU) products - declared as follows:
Specification. - This article contains substances listed in the
candidate list (date: 31.08.2022) exceeding 0.1
The declaration of performance of the product can be percentage by mass: no.
found at www.kingspan.com. - This article contains other carcinogenic, mutagenic,
reprotoxic (CMR) substances in categories 1A or 1B
Base materials/Ancillary materials which are not on the candidate list, exceeding 0.1
The product contains approximately 0,6 kg/m2 percentage by mass: no.
polyurethane rigid foam and 0,3 kg/m2 multi-layer - Biocide products were added to this construction
aluminium facings. product or it has been treated with biocide products
(this then concerns a treated product as defined by the
The main materials of the polyurethane foam are MDI (EU) Biocidal Products Regulation No. 528/2012
(between 57-62 %), polyol (between 27-32 %) and a (BPR): no.
blowing agent (between 5-6 %). Due to the closed-cell
structure (conform EN 13165), the blowing agent Reference service life
remains in the foam. Water, flame retardants and The reference service life is not to be declared in this
additives are added (between 4-8 %). EPD as it does not cover the use stage.
In the current REACH regulations, polyurethane foam
insulation products are considered “articles” and are
LCA: Calculation rules
Declared Unit · A4 transport to the building site;
The declared unit (1 m²) and conversion factors are · A5 installation in the building including provision of all
listed in the table below. materials, products and energy, as well as waste
processing up to the end-of-waste state or disposal of
Declared unit final residues during the construction process stage.
Name Value Unit
Declared unit 1 m2 The end-of-life stage is a mandatory information
Gross density 30 kg/m3 module and it covers:
Grammage 0.9 kg/m2 · C1 de-construction, demolition;
Layer thickness 0.03 m · C2 transport to waste processing;
· C3 waste processing for reuse, recovery and/or
The scope of this EPD is the thermal insulation recycling;
product Kingspan Sauna-Satu® as produced by · C4 disposal (not applicable for this EPD) including
Kingspan Insulation at the manufacturing facility in provision and all transport, provision of all materials,
Kankaanpää (Finland). The environmental impacts products and related energy and water use.
have been calculated over the calendar year 2021.
Environmental burden of the incineration (R1 > 60 %)
The EPD is studied for a product thickness of 30 mm. of the product
at the end-of-life stage are assigned to the product
system (C3); resulting potential credits for thermal and
electrical energy from energy substitution are declared
System boundary in module D.
The type of EPD according to EN 15804 is:
cradle to gate with options, modules C1–C4, and Comparability
module D (A1–A3, C, D and additional modules: Basically, a comparison or an evaluation of EPD data
A4, A5). is only possible if all the data sets to be compared
were created according to EN 15804 and the building
The product stage is a mandatory information module context, respectively the product-specific
and it covers: characteristics of performance, are taken into account.
· A1, raw material extraction and processing,
processing of secondary material input (e.g. recycling
processes), Background database
· A2, transport to the manufacturer, Background data from GaBi ts Version 10 is used with
· A3, manufacturing, including provision of all GaBi data sets CUP2022.1.
materials, products and energy, packaging processing
and its transport, as well as waste processing up to the
end-of-waste state or disposal of final residues
during the product stage.
The construction process stage includes:
3 Environmental Product Declaration Kingspan Insulation B.V. – Kingspan Sauna-Satu®
LCA: Scenarios and additional technical information
Characteristic product properties
Information on biogenic carbon
The total mass of biogenic carbon containing materials
is less than 5 % of the total mass of the product and
accompanying packaging.
Technical information
The following technical information is a basis for the
declared modules or can be used for developing
specific scenarios in the context of a building
assessment.
Manufacturing (A3)
A polyethylene packaging foil is used. The products
are transported either on wooden pallets.
Within Module A3 the following packaging of the final
product is included:
- Polyethylene cover and wrap: 0,009 kg/m²
- Expanded Polystyrene skid: 0,000 kg/m²
- Wooden pallet: 0,017 kg/m²
Transport to the building site (A4)
Name Value Unit
Litres of fuel 0.0103 l/100km
Transport distance 100 km
Gross density of products
30 kg/m3
transported
Installation into the building (A5)
Name Value Unit
Output substances following
0.027 kg
waste treatment on site
The recycling of the packaging is considered in A5.
End of life (C1-C4)
The assumptions for C1 are: diesel driven excavator
(100 kW; 0.2 litre fuel per ton excavated material). The
assumptions for C2 are: Truck Euro 6, diesel driven,
26-28 t gross weight, assumed distance 50 km
Name Value Unit
Collected as mixed construction
0.9 kg
waste
Energy recovery 0.875 kg
Recycling (aluminium content of
0.025 kg
the multi-layer aluminium facings)
Reuse, recovery and/or recycling potentials (D),
relevant scenario information
Waste incineration with energy recuperation is
assumed as end-of-life scenario
4 Environmental Product Declaration Kingspan Insulation B.V. – Kingspan Sauna-Satu®
LCA: Results
DESCRIPTION OF THE SYSTEM BOUNDARY (X = INCLUDED IN LCA; ND = MODULE OR INDICATOR NOT
DECLARED; MNR = MODULE NOT RELEVANT)
BENEFITS AND
CONSTRUCTI LOADS
PRODUCT STAGE ON PROCESS USE STAGE END OF LIFE STAGE BEYOND THE
STAGE SYSTEM
BOUNDARIES
5 Environmental Product Declaration Kingspan Insulation B.V. – Kingspan Sauna-Satu®
lairetam
waR
ylppus tropsnarT
gnirutcafunaM
eht
morf
tropsnarT
etis
eht
ot
etag
ylbmessA esU
ecnanetniaM
riapeR
tnemecalpeR tnemhsibrufeR
ygrene
lanoitarepO esu
retaw
lanoitarepO esu
noitcurtsnoc-eD
noitilomed tropsnarT
gnissecorp
etsaW
lasopsiD -esueR -yrevoceR -gnilcyceR laitnetop
A1 A2 A3 A4 A5 B1 B2 B3 B4 B5 B6 B7 C1 C2 C3 C4 D
X X X X X ND ND MNR MNR MNR ND ND X X X X X
RESULTS OF THE LCA - ENVIRONMENTAL IMPACT according to EN 15804+A2: 1m2 30mm Kingspan
Sauna-Satu®
Core Indicator Unit A1-A3 A4 A5 C1 C2 C3 C4 D
GWP-total [kg CO2-Eq.] 2.45E+0 7.58E-3 5.34E-2 5.77E-4 3.79E-3 1.84E+0 0.00E+0 -8.47E-1
GWP-fossil [kg CO2-Eq.] 2.67E+0 7.54E-3 2.29E-2 5.77E-4 3.77E-3 1.67E+0 0.00E+0 -8.43E-1
GWP-biogenic [kg CO2-Eq.] -2.19E-1 -1.04E-5 3.05E-2 7.72E-7 -5.21E-6 1.66E-1 0.00E+0 -3.83E-3
GWP-luluc [kg CO2-Eq.] 1.68E-3 4.21E-5 3.25E-7 7.12E-9 2.10E-5 3.71E-6 0.00E+0 -1.06E-4
ODP [kg CFC11-Eq.] 5.71E-12 4.52E-16 6.31E-15 3.54E-17 2.26E-16 1.41E-13 0.00E+0 -4.58E-12
AP [mol H+-Eq.] 6.04E-3 7.78E-6 7.15E-6 2.68E-6 3.89E-6 1.03E-3 0.00E+0 -1.81E-3
EP-freshwater [kg P-Eq.] 1.20E-5 2.25E-8 1.56E-9 1.16E-10 1.13E-8 3.87E-8 0.00E+0 -9.76E-7
EP-marine [kg N-Eq.] 1.50E-3 2.54E-6 2.18E-6 1.28E-6 1.27E-6 4.93E-4 0.00E+0 -3.45E-4
EP-terrestrial [mol N-Eq.] 1.57E-2 3.03E-5 3.35E-5 1.40E-5 1.51E-5 5.69E-3 0.00E+0 -3.71E-3
POCP [kg NMVOC-Eq.] 6.67E-3 6.85E-6 6.03E-6 3.62E-6 3.43E-6 1.27E-3 0.00E+0 -1.00E-3
ADPE [kg Sb-Eq.] 1.90E-6 6.31E-10 1.54E-10 2.36E-11 3.15E-10 3.82E-9 0.00E+0 -1.12E-7
ADPF [MJ] 6.52E+1 1.01E-1 1.47E-2 7.80E-3 5.04E-2 4.81E-1 0.00E+0 -1.35E+1
[m³ world-Eq
WDP 3.57E-1 6.77E-5 5.32E-3 1.07E-6 3.39E-5 1.85E-1 0.00E+0 -9.99E-2
deprived]
GWP = Global warming potential; ODP = Depletion potential of the stratospheric ozone layer; AP = Acidification potential of land and water; EP =
Caption Eutrophication potential; POCP = Formation potential of tropospheric ozone photochemical oxidants; ADPE = Abiotic depletion potential for non-
fossil resources; ADPF = Abiotic depletion potential for fossil resources; WDP = Water (user) deprivation potential
RESULTS OF THE LCA - INDICATORS TO DESCRIBE RESOURCE USE according to EN 15804+A2: 1m2
30mm Kingspan Sauna-Satu®
Indicator Unit A1-A3 A4 A5 C1 C2 C3 C4 D
PERE [MJ] 1.03E+1 5.73E-3 2.59E-1 2.95E-5 2.87E-3 8.65E-2 0.00E+0 -4.21E+0
PERM [MJ] 2.55E-1 0.00E+0 -2.55E-1 0.00E+0 0.00E+0 0.00E+0 0.00E+0 0.00E+0
PERT [MJ] 1.06E+1 5.73E-3 3.61E-3 2.95E-5 2.87E-3 8.65E-2 0.00E+0 -4.21E+0
PENRE [MJ] 3.72E+1 1.01E-1 4.02E-1 7.82E-3 5.05E-2 2.81E+1 0.00E+0 -1.35E+1
PENRM [MJ] 2.80E+1 0.00E+0 -3.87E-1 0.00E+0 0.00E+0 -2.77E+1 0.00E+0 0.00E+0
PENRT [MJ] 6.53E+1 1.01E-1 1.47E-2 7.82E-3 5.05E-2 4.81E-1 0.00E+0 -1.35E+1
SM [kg] 0.00E+0 0.00E+0 0.00E+0 0.00E+0 0.00E+0 0.00E+0 0.00E+0 0.00E+0
RSF [MJ] 0.00E+0 0.00E+0 0.00E+0 0.00E+0 0.00E+0 0.00E+0 0.00E+0 0.00E+0
NRSF [MJ] 0.00E+0 0.00E+0 0.00E+0 0.00E+0 0.00E+0 0.00E+0 0.00E+0 0.00E+0
FW [m³] 1.95E-2 6.48E-6 1.26E-4 4.44E-8 3.24E-6 4.35E-3 0.00E+0 -5.85E-3
PERE = Use of renewable primary energy excluding renewable primary energy resources used as raw materials; PERM = Use of
renewable primary energy resources used as raw materials; PERT = Total use of renewable primary energy resources; PENRE = Use of
non-renewable primary energy excluding non-renewable primary energy resources used as raw materials; PENRM = Use of non-
Caption
renewable primary energy resources used as raw materials; PENRT = Total use of non-renewable primary energy resources; SM = Use
of secondary material; RSF = Use of renewable secondary fuels; NRSF = Use of non-renewable secondary fuels; FW = Use of net fresh
water
RESULTS OF THE LCA – WASTE CATEGORIES AND OUTPUT FLOWS according to EN 15804+A2:
1m2 30mm Kingspan Sauna-Satu®
Indicator Unit A1-A3 A4 A5 C1 C2 C3 C4 D
HWD [kg] 4.39E-8 4.84E-13 1.31E-12 2.58E-14 2.42E-13 6.44E-11 0.00E+0 -1.21E-9
NHWD [kg] 1.17E-1 1.45E-5 2.24E-3 7.32E-7 7.24E-6 1.37E-2 0.00E+0 -6.02E-2
RWD [kg] 1.45E-3 1.25E-7 7.22E-7 8.57E-9 6.23E-8 2.05E-5 0.00E+0 -1.03E-3
CRU [kg] 0.00E+0 0.00E+0 0.00E+0 0.00E+0 0.00E+0 0.00E+0 0.00E+0 0.00E+0
MFR [kg] 0.00E+0 0.00E+0 0.00E+0 0.00E+0 0.00E+0 2.54E-2 0.00E+0 0.00E+0
MER [kg] 0.00E+0 0.00E+0 2.60E-2 0.00E+0 0.00E+0 7.55E-1 0.00E+0 0.00E+0
EEE [MJ] 0.00E+0 0.00E+0 8.53E-2 0.00E+0 0.00E+0 2.88E+0 0.00E+0 0.00E+0
EET [MJ] 0.00E+0 0.00E+0 1.53E-1 0.00E+0 0.00E+0 5.15E+0 0.00E+0 0.00E+0
HWD = Hazardous waste disposed; NHWD = Non-hazardous waste disposed; RWD = Radioactive waste disposed; CRU = Components
Caption for re-use; MFR = Materials for recycling; MER = Materials for energy recovery; EEE = Exported electrical energy; EET = Exported
thermal energy
RESULTS OF THE LCA – additional impact categories according to EN 15804+A2-optional:
1m2 30mm Kingspan Sauna-Satu®
Indicator Unit A1-A3 A4 A5 C1 C2 C3 C4 D
[Disease
PM 5.62E-8 4.49E-11 5.56E-11 3.03E-11 2.25E-11 2.98E-9 0.00E+0 -1.71E-8
Incidence]
[kBq U235-
IRP 1.85E-1 1.83E-5 1.09E-4 1.25E-6 9.12E-6 3.29E-3 0.00E+0 -1.80E-1
Eq.]
ETP-fw [CTUe] 2.73E+1 7.00E-2 8.75E-3 5.43E-3 3.50E-2 1.71E-1 0.00E+0 -3.31E+0
HTP-c [CTUh] 1.82E-9 1.41E-12 5.24E-13 1.01E-13 7.06E-13 1.24E-11 0.00E+0 -2.26E-10
HTP-nc [CTUh] 1.51E-7 7.32E-11 4.04E-11 5.08E-12 3.66E-11 4.60E-10 0.00E+0 -6.65E-9
SQP [-] 3.78E+1 3.47E-2 4.01E-3 2.15E-5 1.74E-2 1.04E-1 0.00E+0 -2.07E+0
PM = Potential incidence of disease due to PM emissions; IR = Potential Human exposure efficiency relative to U235; ETP-fw = Potential
Caption comparative Toxic Unit for ecosystems; HTP-c = Potential comparative Toxic Unit for humans (cancerogenic); HTP-nc = Potential
comparative Toxic Unit for humans (not cancerogenic); SQP = Potential soil quality index
Disclaimer 1 – for the indicator “Potential Human exposure efficiency relative to U235”.This impact category deals
mainly with the eventual impact of low-dose ionizing radiation on human health of the nuclear fuel cycle. It does
not consider effects due to possible nuclear accidents, occupational exposure or to radioactive waste disposal in
underground facilities. Potential ionizing radiation from the soil, radon and from some construction materials is
also not measured by this indicator.
Disclaimer 2 – for the indicators “abiotic depletion potential for non-fossil resources”, “abiotic depletion potential
for fossil resources”, “water (user) deprivation potential, deprivation-weighted water consumption”, “potential
comparative toxic unit for ecosystems”, “potential comparative toxic unit for humans – cancerogenic”, “Potential
comparative toxic unit for humans - not cancerogenic”, “potential soil quality index”. The results of this
environmental impact indicator shall be used with care as the uncertainties on these results are high as there is
limited experience with the indicator.
References
Biocidal Products Regulation No. 528/2012 (BPR) www.ibu-epd.com
Regulation (EU) No 528/2012 of the European
Parliament and of the Council of 22 May 2012 LCA-tool
concerning the making available on the market and Kingspan LCA tool, version 1.1. IBU-KSI-202001-LT1-
use of biocidal products EN.
Developed by Sphera Solutions GmbH (formely
CPR Thinkstep GmbH)
Regulation (EU) No. 305/2011 of the European
Parliament and of the Council of 9 March 2011 laying PCR Version 1.7, Part A
down harmonised condition for the marketing of Institut Bauen und Umwelt e.V., Berlin (pub.): Product
construction products and repealing Council Directive Category Rules for Building-Related Products and
89/106/EC services, Part A: Calculation Rules for the Life Cycle
Assessment and Requirements on the Project Report
ISO 14025 according to EN 15804+A2:2019
EN ISO 14025:2011, Environmental labels and November 2021
declarations — Type III environmental declarations —
Principles and procedures. PCR 2017, Part B
Institut Bauen und Umwelt e.V., Berlin (pub.): Product
EN 13165 Category Rules for Construction Products from the
EN 13165:2012+A2:2016: Thermal insulation products range of Environmental Product Declarations of Institut
for buildings. Factory made polyurethane foam (PU) Bauen und Umwelt (IBU), Part B: Requirements on the
products. Specification EPD for insulating materials made of foam
plastics. January 2019
EN 15804
EN 15804:2012+A2:2019+AC:2021, Sustainability of REACH
construction works — Environmental Product Regulation (EC) No 1907/2006 of the European
Declarations — Core rules for the product category of Parliament and of the Council on the Registration,
construction products. Evaluation, Authorisation and Restriction of Chemicals
(REACH)
GaBi ts https://echa.europa.eu/candidate-list-table;
thinkstep AG: Leinfelden-Echterdingen GaBi Software-
System and Database for Life Cycle Engineering 1992- Candidate list
2019 https://echa.europa.eu/candidate-list-table; accessed
31.08.2022, 233 substances listed.
IBU 2021
Institut Bauen und Umwelt e.V.: General Instructions
for the EPD programme of Institut Bauen und Umwelt
e.V., Version 2.0, Berlin: Institut Bauen und Umwelt
e.V., 2021.
6 Environmental Product Declaration Kingspan Insulation B.V. – Kingspan Sauna-Satu®
Publisher
Institut Bauen und Umwelt e.V. Tel +49 (0)30 3087748- 0
Hegelplatz 1 Fax +49 (0)30 3087748- 29
10117 Berlin Mail info@ibu-epd.com
Germany Web www.ibu-epd.com
Programme holder
Institut Bauen und Umwelt e.V. Tel +49 (0)30 - 3087748- 0
Hegelplatz 1 Fax +49 (0)30 – 3087748 - 29
10117 Berlin Mail info@ibu-epd.com
Germany Web www.ibu-epd.com
Author of the Life Cycle
Assessment Tel +31 (0) 543 543 210
Kingspan Insulation B.V. Fax +31 (0) 344 675 251
Lingewei 8 Mail info@kingspaninsulation.nl
4004LL Tiel Web www.kingspan.com
Netherlands
Owner of the Declaration
Kingspan Insulation B.V. Tel +31 (0) 543 543 210
Lingewei 8 Fax +31 (0) 344 675 251
4004LL Tiel Mail info@kingspaninsulation.nl
Netherlands Web www.kingspan.com
