ENVIRONMENTAL PRODUCT DECLARATION
as per ISO 14025 and EN 15804+A2
Owner of the Declaration Knauf Gips KG
Publisher Institut Bauen und Umwelt e.V. (IBU)
Programme holder Institut Bauen und Umwelt e.V. (IBU)
Declaration number EPD-KNA-20230175-IBA1-EN
Issue date 14.08.2023
Valid to 13.08.2028
Knauf Safeboard GKF
Knauf Gips KG
www.ibu-epd.com | https://epd-online.com
1. General Information
Knauf Gips KG Knauf Safeboard GKF
Programme holder Owner of the declaration
IBU – Institut Bauen und Umwelt e.V. Knauf Gips KG
Hegelplatz 1 Am Bahnhof 7
10117 Berlin 97346 Iphofen
Germany Germany
Declaration number Declared product / declared unit
EPD-KNA-20230175-IBA1-EN Plasterboard Knauf Safeboard Type GKF according to DIN 18180
respectively DF according to EN 520, 1 m², board thickness 12.5 mm,
weight of board approx. 17.7 kg/m²
This declaration is based on the product category rules: Scope:
Plasterboard, 11.07.2023 This EPD covers 100 % of manufacture of the plasterboard Knauf
(PCR checked and approved by the SVR) Safeboard GKF. This plasterboard is manufactured in Germany. The life
cycle assessment is based on production data for 2021/22.
The owner of the declaration shall be liable for the underlying information
Issue date and evidence; the IBU shall not be liable with respect to manufacturer
information, life cycle assessment data and evidences.
14.08.2023
The EPD was created according to the specifications of EN 15804+A2. In
the following, the standard will be simplified as EN 15804.
Valid to
13.08.2028 Verification
The standard EN 15804 serves as the core PCR
Independent verification of the declaration and data according to ISO
14025:2011
internally X externally
Dipl.-Ing. Hans Peters
(Chairman of Institut Bauen und Umwelt e.V.)
Florian Pronold Ms Jane Anderson,
(Managing Director Institut Bauen und Umwelt e.V.) (Independent verifier)
1 Environmental Product Declaration - Knauf Gips KG - Knauf Safeboard GKF
2. Product
Further information is available in the technical data sheet
2.1 Product description/Product definition K762.de_ENG Knauf Safeboard GKF under www.knauf.de.
Plasterboard Knauf Safeboard GKF is a lead-free X-ray
shielding board for X-ray equipment designed to shield against Performance data of the product in accordance with the
radiation for enhanced stability and higher fire resistance declaration of performance with respect to its essential
quality. characteristics according to EN 520.
For the placing on the market of the product in the European
Union/European Free Trade Association (EU/EFTA) (with the 2.4 Delivery status
exception of Switzerland) Regulation (EU) No. 305/2011 Plasterboards Knauf Safeboard GKF according to DIN 18180
CPR2011 applies. The product Knauf Safeboard GKF 12.5 mm (Type DF according to EN 520) are delivered with a board
needs a declaration of performance and the CE-marking thickness of 12.5 mm as well as a size of 2500 mm x 625 mm
harmonized acc. to EN 520. with a half-rounded long edge (HRAK) and front cut square
edge (SSK).
For the application and use the respective national provisions
2.5 Base materials/Ancillary materials
apply.
Knauf Safeboard GFK consists of more than 90 % of set
2.2 Application gypsum and baryte, covered with a board liner (< 3 %).
Knauf Safeboard GKF are used for room-enclosing Furthermore, the plasterboards contain small amounts (< 5 %)
constructions of X-ray facilities for radiation shielding regarding of starch, tensides, fibre additives as well as in-organic colour
the following systems: pigments.
• X-Ray shield suspended ceilings
The declared products contain substances listed in the
• X-Ray shield partitions
candidate list (date: 14.06.2023, ECHA2023) exceeding 0.1
• X-Ray shield furring
percentage by mass: no.
2.3 Technical Data
The following technical data in condition on delivery is relevant This product contains other CMR substances in categories 1A
for the declared product: or 1B (Regulation (EC) No. 1272/2008) which are not on the
candidate list, exceeding 0.1 percentage by mass: no
Constructional data
Name Value Unit Biocide products were added to this construction product or it
Gross density ≥ 1400 kg/m3 has been treated with biocide products (this then concerns a
treated product as defined by the (EU) Ordinance on Biocide
Flexural breaking load longitudinal according
≥ 610 N Products No. 528/2012): no
to DIN 18180
Flexural breaking load transversal according 2.6 Manufacture
≥ 210 N
to DIN 18180
The manufacturing process for gypsum boards is shown in
Thermal conductivity following EN 12664 0.26 W/(mK) Figure 1:
Water vapour diffusion resistance factor
10 -
(dry), according to EN ISO 10456
Water vapour diffusion resistance factor
4 -
(wet), according to EN ISO 10456
Shrinkage and expansion air humidity per 1 0.005 /
mm/m
% change of relative air humidity 0.008
Shrinkage and expansion temperature per 1 0.013 /
mm/m
Kelvin change of temperature 0.02
2 Environmental Product Declaration - Knauf Gips KG - Knauf Safeboard GKF
Figure 1: Manufacturing process of gypsum boards
2.8 Product processing/Installation
The components of plasterboards Knauf Safeboard GKF are Storage
suspended in water and spread on a continuous sheet of board Plasterboards Knauf Safeboard GKF should be stored indoors
liner (visible face, lower layer). Beforehand, the board liner is under dust-free and dry conditions in a horizontal position.
cut on the sides for edge shaping. The slurry is covered with a
second sheet of board liner (back surface) in the forming station Application
and the edges of the visible face board liner are flipped During application, dust thresholds are to be observed
upwards. On the subsequent board line the gypsum is setting according to TRGS 900 and TRGS 559. The application and
continuously and is dried in a multi-level drier to the permitted installation should follow the instruction sheets provided under
residual moisture level. Drying is followed by the cutting of the www.knauf.de (e.g., K131, K151, K152, K112) respectively the
boards to the desired lengths. Knauf brochure ST02.de_EN Knauf Safeboard - X-ray
Shielding.
All processes within the company are certified according to ISO
9001. Endless filament glass fibres are used in the manufacturing of
plasterboards Knauf Safeboard GKF for enhanced fire
2.7 Environment and health during manufacturing protection. These fibres do not fan out during application and
The production of Knauf Safeboard GKF is subject to the therefore no fibre dusts according to TRGS 521 occur.
German emission control regulations BImSchG. CO emissions
2
2.9 Packaging
are measured due to CO emissions trading. The German
2
Plasterboards Knauf Safeboard GKF are stacked on reusable
manufacturing sites for the production of Knauf Safeboard GKF
pallets and protected with a PE-film. Pallets are re-used,
are certified according to ISO 50001 as well as certified with the
whereas the PE-film is externally recycled.
occupational safety standard 'Systematic Safety' from the
German Social Accident Insurance Institution for the Raw 2.10 Condition of use
Materials and Chemical Industry BG RCI.
Knauf Safeboard GKF are used for suspended ceilings,
partitions and furring for shielding X-rays. They feature high
Gypsum from the flue-gas desulphurization plants of coal-fired
levels of robustness against mechanical impacts and serve
power stations is used in addition to natural gypsum.
increased demands on fire protection. There is no change in
Production waste as well as dust from the filtration units are
the chemical composition during use.
recycled internally and fed back into the production of
plasterboards. 2.11 Environment and health during use
Knauf Safeboard GKF are able to shield effectively against X-
rays. The respective values of lead equivalence according to
3 Environmental Product Declaration - Knauf Gips KG - Knauf Safeboard GKF
DIN 6812 are available in the technical data sheet under exchange of heavily damaged boards. In this case, the
www.knauf.de. substructure should be examined, too, and replaced if
necessary.
According to the emission test of Eurofins Product Testing A/S
Eurofins2021, no hazardous substances are emitted above 2.14 Re-use phase
permissible thresholds during use. Re-use
Once plasterboards Knauf Safeboard GKF are installed, they
2.12 Reference service life are not suited for re-use in an unchanged way. Prior to
There was no reference service life determined according to collection, plasterboards Knauf Safeboard GKF should be
ISO 15686-1. However, a reference service life of 50 years can separated from other used building materials and pruned of
be considered for gypsum plasterboards according to the foreign matter, e.g., metals from the substructure already on
Guideline for Sustainable Building BBSR2017. There are no site for easier recycling or disposal.
influences on ageing of plasterboards Knauf Safeboard GKF
during use following the established engineering practice. Further use
Residual materials from new plasterboards Knauf Safeboard
2.13 Extraordinary effects GKF, e.g., from cut waste at the building site, can be disposed
Fire of at a landfill.
The reaction to fire of plasterboards Knauf Safeboard GKF is
classified as follows according to EN 520 in conjunction with EN Recycling
13501-1. In principle, gypsum boards can be recycled by standard
Fire safety regulations recycling processes. However, Knauf Safeboard GKF is not
suitable for recycling due to the barytes included int the gypsum
Name Value
core.
Building material class ; fire behaviour class A2
Smoke gas development ; smoke production s1 2.15 Disposal
Burning droplets ; flaming droplets/particles d0 X-ray shielding boards Knauf Safeboard GKF have to be
disposed of in compliance with the following waste codes of the
A2 = non-combustible
European Waste Catalogue EWC:
s1 = no smoke
d0 = no burning fall-off/drop-off
17 08 02 - gypsum-based construction materials other than
those mentioned in 17 08 01
17 09 04 - mixed construction and demolition wastes other than
Water
those mentioned in 17 09 01, 17 09 02 and 17 09 03
Knauf Safeboard GKF show a small tendency to swell or shrink
within changes of climatic conditions. However, a permanent
National disposal guidelines need to be observed. In Germany,
exposure to wet conditions or very high levels of relative
plasterboards Knauf Safeboard GKF are to be disposed of at
humidity may lead to a decrease in strength. An instruction
landfills of landfill category 1 or higher according to the
sheet about the restoration of flood damage is available under
regulation of landfills DepV2021.
www.knauf.de BSDH2013.
2.16 Further information
Mechanical destruction Further information about plasterboards Knauf Safeboard GKF,
Minor damages on Knauf Safeboard GKF can be mended with e.g., technical data sheets or material safety data sheets are
suitable gypsum-based filling materials, e.g., Knauf Safeboard available at www.knauf.de.
Filler. The installation with screws and brackets allows an easy
3. LCA: Calculation rules
• transport to building site (A4)
3.1 Declared Unit • installation at building site (A5) including the incineration
The declared unit is 1 m² of plasterboard Knauf Safeboard GKF of transport packaging
with a thickness of 12.5 mm, weight approx. 17.7 kg/m². • disassembly (C1)
Declared Unit • transport to recycling facility or landfill site (C2)
• landfilling at end of life (C4)
Name Value Unit
• credits in D from incineration of packaging material in A5
Declared unit 1 m2 The life cycle of Knauf Safeboard GKF is outlined in Figure 2.
Conversion factor to 1 kg 0.056 -
Other declared units are allowed if the conversion is shown
transparently.
3.2 System boundary
Type of the EPD: cradle to gate - with options, modules C1–C4,
and module D (A1–A3 + C+ D, additional modules: A4, A5)
This Environmental Product Declaration according to EN 15804
contains:
• provision of raw materials and transport to plant,
production of boards (A1-A3) including thermal energy
for calcination and drying (from natural gas, geographic
scope: DE), as well as electricity (residual mix DE)
4 Environmental Product Declaration - Knauf Gips KG - Knauf Safeboard GKF
3.5 Background data
For modelling the LCA the software LCA for Experts with data
base version 2023.1 from Sphera is used. Data sets for
Germany are used for the life cycle inventory as much as
possible. This is especially true for the provision of electricity
and thermal energy for processes inside the Knauf plant.
3.6 Data quality
The LCA of plasterboards Knauf Safeboard GKF is modelled by
using LCA for Experts, exclusively. All datasets used have been
updated in the last 5 years. For processes and materials, where
no direct match is available, data from literature or expert
judgements are applied. Only a few materials and processes
needed to be cut off due to missing information. Since these
Figure 2: Principal life cycle of gypsum boards cut-off materials and processes are only of small amounts (<< 1
% w/w), the total influence of these neglected inputs is
expected to be lower than 5 % of energy usage and mass.
3.3 Estimates and assumptions
For modelling the manufacturing of Knauf Safeboard GKF in With respect to technological, geographic and time
plant Iphofen, the residual electricity for Germany has been representativeness, the overall data quality is evaluated to be
chosen, whereas processes beyond the plant gate were mainly 'satisfactory'.
modelled with the European electricity consumption mix.
3.7 Period under review
Some raw materials and additives were not available in the The modelling of Knauf Safeboard GKF is based on data from
background database and therefore were either substituted production years 2021/2022. Since different plasterboards are
with similar materials or modelled with their own processes. manufactured subsequentially, the energy consumption is
The respectively chosen methods are described in the measured directly during the production of each board type.
background report.
3.8 Geographic Representativeness
Land or region, in which the declared product system is
Transport to the building site (module A4) as well as transport
manufactured, used or handled at the end of the product´s
from the building site to landfill (module C2) is calculated with a
lifespan: Global
standard distance of 100 km. This way, the user of the
Environmental Product Declaration can convert the distances of
modules A4 and C2 to the specific distance by extrapolation.
3.9 Allocation
3.4 Cut-off criteria Allocations are avoided in the modelling of production data.
There may be allocations in the background data which are are
All raw materials for the manufacturing of plasterboards Knauf
explained in the documentation of the respective datasets.
Safeboard GKF, the required energy, water and the resulting
emissions are considered in the life cycle assessment. That
3.10 Comparability
way, recipe components with a share even smaller than 1 %
Basically, a comparison or an evaluation of EPD data is only
are included.
possible if all the data sets to be compared were created
Cut-off rules as required by EN 15804+A2 are respected. The
according to EN 15804 and the building context, respectively
details are given in the background report. The environmental
the product-specific characteristics of performance, are taken
impacts imposed by these cut-offs are considered neglectable.
into account.
All neglected processes contribute less than 5 % to the total
mass or less than 5 % to the total energy consumption.
4. LCA: Scenarios and additional technical information
mainly extracted from open-cast mining in close vicinity to the
Characteristic product properties of biogenic carbon manufacturing site. Furthermore, gypsum from the flue-gas
Information on describing the biogenic carbon content at desulphurization of coal-fired power stations (FGD gypsum) is
factory gate used as a raw material. Board liner for the covering of gypsum
core is produced from recycled waste paper which is certified
Name ValueUnit
by FSC and/or PEFC. Additives are added for an easier
kg
Biogenic carbon content in product 0.211 processing and a fine adjustment of properties of plasterboards
C
Knauf Safeboard GKF. These additives add up to less than 5 %
Biogenic carbon content in accompanying kg of the overall mass of the product.
0.043
packaging C
Transport of raw materials
Natural gypsum is extracted from mines close to the
Product Stage (A1-A3)
manufacturing sites of plasterboard Knauf Safeboard GKF.
Accordingly, transport distances are short and trucks can be
Supply of raw materials
used. FGD gypsum is transported by freight train from coal-fired
Plasterboards Knauf Safeboard GKF consist of a gypsum core
power plants. The heavy spar is produced predominantly in
and barytes which is reinforced with mineral fillers and covered
Germany and also delivered by truck. In parts, baryte can also
with board liner. For its identification the core of Knauf
be delivered from overseas by container ship. Further raw
Safeboard GKF is coloured in yellow. The natural gypsum is
5 Environmental Product Declaration - Knauf Gips KG - Knauf Safeboard GKF
materials are supplied by truck from manufacturers within
Germany or from neighbouring countries. Use phase (B1-B7): Excluded since no environmental
impacts/benefits are expected.
Manufacturing
Natural gypsum as well as gypsum from the flue-gas
desulphurization is calcinated prior to the mixing with other
components. FGD gypsum is usually delivered as damp
End of life (C1-C4)
material and, thus, must be dried before calcination. Stucco,
The demolition (C1) of the Knauf Safeboard GKF from the
mineral fillers and additives are mixed with water and
building is considered to be done 100 % manually. It is
processed as described in section 2.6. The addition of water
assumed that the deconstruction would take place without
allows the incorporation of water of crystallization into the
further processing of the waste.
molecules of calcium sulphate. By the addition of water,
gypsum becomes settled and hardened. Redundant surface
For the transport (C2) from the demolition site to the landfill by
water is removed in a multi-level dryer.
truck, a distance of 100 km was assumed in the calculation.
Transport to building site (A4) Transport (C2)
For transport, a standard distance of 100 km by truck is Name Value Unit
assumed. This declaration facilitates the extrapolation of the
Transport distance 100 km
results in A4 to the real distance.
Capacity utilisation (including empty runs) 61 %
Name Value Unit
Litres of fuel (Diesel, density: 0.83 kg/l) 0.0364 l/100km
Currently, Knauf Safeboard GKF are not recycled. Therefore,
Transport distance 100 km
module C3 is declared with 0 impacts.
Capacity utilisation (including empty runs) 61 %
Gross density of products transported ≥ 1400 kg/m3 Disposal (C4) includes the disposal of Knauf Safeboard GKF at
an inert landfill.
Disposal (C4)
Assembly on building site (A5)
Name Value Unit
The installation in the building includes the electricity
Collected separately 17.7 kg
consumption for fastening the Knauf Safeboard GKF.
Collected as mixed construction waste - kg
Accessories such as screws or the substructure itself are not
part of the LCA in this EPD. The energy consumption for the Reuse - kg
electrical devices was considered with 0.0018 kWh/m². Recycling - kg
Energy recovery - kg
The waste material (0.887 kg/m²) from the construction site is
Landfilling 17.7 kg
transported by truck to a landfill and disposed of. The
replacement of this construction waste is considered in A5 as Reuse-, recover- and recycling potential (D): Module D
well. contains only credits for exported energy from incineration of
packaging material (results only from A5)
The packaging material, re-usable wooden pallets and PE-film,
are incinerated. The credits from this process are reported in
Modul D.
Name Value Unit
Electricity consumption 0.0018 kWh
Material loss (landfilling) 0.887 kg
Reference service life according to BBSR2017 50 a
6 Environmental Product Declaration - Knauf Gips KG - Knauf Safeboard GKF
5. LCA: Results
DESCRIPTION OF THE SYSTEM BOUNDARY (X = INCLUDED IN LCA; MND = MODULE OR INDICATOR NOT DECLARED; MNR
= MODULE NOT RELEVANT)
Benefits and
Construction loads beyond
Product stage Use stage End of life stage
process stage the system
boundaries
la ire ta m w a Ry lp p u s tro p s n a rT g n iru tc a fu n a M e h t m o rf tro p s n a rTe tis e h t o t e ta g y lb m e s s A e s U e c n a n e tn ia M ria p e R tn e m e c a lp e R tn e m h s ib ru fe R y g re n e la n o ita re p Oe s u re ta w la n o ita re p Oe s u n o itc u rts n o c -e Dn o itilo m e d tro p s n a rT g n is s e c o rp e ts a W la s o p s iD -e s u e R-y re v o c e R-g n ilc y c e Rla itn e to p
A1 A2 A3 A4 A5 B1 B2 B3 B4 B5 B6 B7 C1 C2 C3 C4 D
X X X X X MND MND MNR MNR MNR MND MND X X X X X
RESULTS OF THE LCA - ENVIRONMENTAL IMPACT according to EN 15804+A2: 1 m² Knauf Safeboard GKF 12.5 mm; 17.7
kg/m²
Parameter Unit A1-A3 A4 A5 C1 C2 C3 C4 D
GWP-total kg CO 2 eq 1.36E+00 1.31E-01 3.16E-01 0 1.31E-01 0 1.17E+00 -6.36E-02
GWP-fossil kg CO 2 eq 2.3E+00 1.3E-01 1.57E-01 0 1.3E-01 0 2.67E-01 -6.29E-02
GWP-biogenic kg CO 2 eq -9.42E-01 0 1.59E-01 0 0 0 9.01E-01 -6.06E-04
GWP-luluc kg CO 2 eq 2.62E-03 1.18E-03 2.72E-04 0 1.18E-03 0 8.29E-04 -6E-06
ODP kg CFC11 eq 1.43E-11 1.99E-14 7.82E-13 0 1.99E-14 0 6.86E-13 -8.56E-13
AP mol H+ eq 4.36E-03 1.64E-04 3.59E-04 0 1.64E-04 0 1.89E-03 -6.64E-05
EP-freshwater kg P eq 1.67E-05 4.66E-07 9.08E-07 0 4.67E-07 0 5.39E-07 -1.89E-07
EP-marine kg N eq 1.36E-03 5.69E-05 1.07E-04 0 5.7E-05 0 4.89E-04 -2.37E-05
EP-terrestrial mol N eq 1.38E-02 6.68E-04 1.15E-03 0 6.69E-04 0 5.38E-03 -2.51E-04
kg NMVOC
POCP 3.34E-03 1.41E-04 2.79E-04 0 1.42E-04 0 1.48E-03 -6.13E-05
eq
ADPE kg Sb eq 1.83E-07 8.49E-09 1.09E-08 0 8.51E-09 0 1.23E-08 -6.03E-09
ADPF MJ 3.66E+01 1.75E+00 2.25E+00 0 1.75E+00 0 3.55E+00 -9.57E-01
m3 world eq
WDP 6.74E-02 1.6E-03 2.49E-02 0 1.6E-03 0 2.92E-02 -9.27E-04
deprived
GWP = Global warming potential; ODP = Depletion potential of the stratospheric ozone layer; AP = Acidification potential of land and water; EP =
Eutrophication potential; POCP = Formation potential of tropospheric ozone photochemical oxidants; ADPE = Abiotic depletion potential for non-fossil
resources; ADPF = Abiotic depletion potential for fossil resources; WDP = Water (user) deprivation potential)
RESULTS OF THE LCA - INDICATORS TO DESCRIBE RESOURCE USE according to EN 15804+A2: 1 m² Knauf Safeboard GKF
12.5 mm; 17.7 kg/m²
Parameter Unit A1-A3 A4 A5 C1 C2 C3 C4 D
PERE MJ 2.17E+00 1.28E-01 2.14E+00 0 1.28E-01 0 5.81E-01 -4.16E-01
PERM MJ 8.4E+00 0 -1.55E+00 0 0 0 0 0
PERT MJ 1.06E+01 1.28E-01 5.9E-01 0 1.28E-01 0 5.81E-01 -4.16E-01
PENRE MJ 3.63E+01 1.76E+00 2.46E+00 0 1.76E+00 0 3.56E+00 -9.57E-01
PENRM MJ 3.77E-01 0 -2.1E-01 0 0 0 0 0
PENRT MJ 3.67E+01 1.76E+00 2.25E+00 0 1.76E+00 0 3.56E+00 -9.57E-01
SM kg 3.98E-01 0 0 0 0 0 0 0
RSF MJ 0 0 0 0 0 0 0 0
NRSF MJ 0 0 0 0 0 0 0 0
FW m3 1.3E-02 1.42E-04 1.18E-03 0 1.42E-04 0 8.96E-04 -1.47E-04
PERE = Use of renewable primary energy excluding renewable primary energy resources used as raw materials; PERM = Use of renewable primary
energy resources used as raw materials; PERT = Total use of renewable primary energy resources; PENRE = Use of non-renewable primary energy
excluding non-renewable primary energy resources used as raw materials; PENRM = Use of non-renewable primary energy resources used as raw
materials; PENRT = Total use of non-renewable primary energy resources; SM = Use of secondary material; RSF = Use of renewable secondary fuels;
NRSF = Use of non-renewable secondary fuels; FW = Use of net fresh water
RESULTS OF THE LCA – WASTE CATEGORIES AND OUTPUT FLOWS according to EN 15804+A2:
1 m² Knauf Safeboard GKF 12.5 mm; 17.7 kg/m²
Parameter Unit A1-A3 A4 A5 C1 C2 C3 C4 D
HWD kg 2.98E-09 9E-12 1.54E-10 0 9.01E-12 0 7.66E-11 -5.27E-12
NHWD kg 5.21E-01 2.71E-04 9.21E-01 0 2.72E-04 0 1.78E+01 -5.43E-04
RWD kg 9.8E-04 3.43E-06 5.58E-05 0 3.43E-06 0 4E-05 -4.31E-05
CRU kg 0 0 0 0 0 0 0 0
MFR kg 0 0 0 0 0 0 0 0
MER kg 0 0 0 0 0 0 0 0
EEE MJ 0 0 2.58E-01 0 0 0 0 0
EET MJ 0 0 4.65E-01 0 0 0 0 0
7 Environmental Product Declaration - Knauf Gips KG - Knauf Safeboard GKF
HWD = Hazardous waste disposed; NHWD = Non-hazardous waste disposed; RWD = Radioactive waste disposed; CRU = Components for re-use;
MFR = Materials for recycling; MER = Materials for energy recovery; EEE = Exported electrical energy; EET = Exported thermal energy
RESULTS OF THE LCA – additional impact categories according to EN 15804+A2-optional:
1 m² Knauf Safeboard GKF 12.5 mm; 17.7 kg/m²
Parameter Unit A1-A3 A4 A5 C1 C2 C3 C4 D
Disease
PM 2.21E-07 1.2E-09 1.26E-08 0 1.2E-09 0 2.33E-08 -5.38E-10
incidence
IR kBq U235 eq 1E-01 5.03E-04 6.01E-03 0 5.04E-04 0 4.54E-03 -4.56E-03
ETP-fw CTUe 1.1E+01 1.24E+00 8.02E-01 0 1.24E+00 0 1.94E+00 -1.87E-01
HTP-c CTUh 5.45E-10 2.53E-11 4.69E-11 0 2.53E-11 0 2.99E-10 -1.25E-11
HTP-nc CTUh 3.75E-08 1.35E-09 3.79E-09 0 1.35E-09 0 3.28E-08 -3.37E-10
SQP SQP 3.6E+01 7.25E-01 1.93E+00 0 7.26E-01 0 8.96E-01 -2.89E-01
PM = Potential incidence of disease due to PM emissions; IR = Potential Human exposure efficiency relative to U235; ETP-fw = Potential comparative
Toxic Unit for ecosystems; HTP-c = Potential comparative Toxic Unit for humans (cancerogenic); HTP-nc = Potential comparative Toxic Unit for humans
(not cancerogenic); SQP = Potential soil quality index
Disclaimer 1 – for the indicator “Potential Human exposure efficiency relative to U235”. This impact category deals mainly with the
eventual impact of low-dose ionizing radiation on human health of the nuclear fuel cycle. It does not consider effects due to possible
nuclear accidents, occupational exposure or radioactive waste disposal in underground facilities. Potential ionizing radiation from the
soil, radon and from some construction materials is also not measured by this indicator.
Disclaimer 2 – for the indicators “abiotic depletion potential for non-fossil resources”, “abiotic depletion potential for fossil resources”,
“water (user) deprivation potential, deprivation-weighted water consumption”, “potential comparative toxic unit for ecosystems”,
“potential comparative toxic unit for humans – cancerogenic”, “Potential comparative toxic unit for humans - not cancerogenic”,
“potential soil quality index”. The results of this environmental impact indicator shall be used with care as the uncertainties on these
results are high as there is limited experience with the indicator.
6. LCA: Interpretation
In general, the highest environmental impacts of Knauf biogenic carbon incorporated in the plasterboard.
Safeboard GKF result from the product stage A1-A3. Landfilling in C4 contributes also considerably to the impact
Exceptions are Global Warming Potential – total GWP-t, non- categories Water deprivation potential WDP (20 %),
hazardous waste disposed NHWD, and Human toxicity - non- Eutrophication – freshwater EP-fw (24 %), Eutrophication –
cancer effects HTP-nc. For those indicators, module C4 and the marine EP-m (25 %), Eutrophication – terrestrial (28 %),
disposal of the boards at inert landfill lead to the highest overall Acidification potential AP (27 %), and Human toxicity - cancer
contributions. effects HTP-c (32 %).
In modules A1-A3, major contributions result from the provision Transports in A4 and in C2 cause only minor contributions to
of raw materials by at least 31 % to the overall life cycle the overall life cycle impacts, due to assumed distances of 100
impacts of the product. Exceptions are Non-hazardous waste km in both modules. Exceptions are Ecotoxicity, freshwater
disposed NHWD (< 1 %), Potential soil quality index SQP ETP-fw (approx. 8 %) and the Global Warming Potential land
(approx. 28 %), and Global Warming Potential land use and use and land use change GWP-luluc (approx. 20 %).
land use change GWP-luluc (approx. 16 %).
Some small credits given in module D result from the
The non-hazardous waste disposed NHWD, is dominated by incineration and recycling of packaging only. The disassembled
the disposal C4 by almost 92 %. This was expected since there product is landfilled after disassembly.
is no recycling at end of life but a complete landfilling. The high
contribution of C4 to GWP-t results from the emission of
7. Requisite evidence
7.1 Leaching (sulphates and heavy metals)
Plasterboards Knauf Safeboard GKF show a leaching 7.3 VOC emissions
behaviour typical for gypsum based building products According to emission test from Eurofins Product Testing A/S,
/Dre2006/. Thus, sulphates are leached in the saturation region no hazardous substances are emitted above permissible
(complexometric titration according to /DIN 38404-5:1985/). thresholds during use /Eurofins2021/.
That is why disposal is only allowed in landfills from landfill
Test after 3 days (limit value)
category 1 in Germany /DepV2009/.
Name Value Unit
Heavy metal concentrations were verified (by ICPOES
according to /ISO 11885:2007/) significantly below the TVOC ≤ 10 mg/m³
assignment criteria according to landfill category 1 complying Total carcinogens < 0.01 mg/m³
with /DepV2009/.
Test after 28 days (limit value)
Plasterboards Knauf Safeboard GKF are classified in water
hazard class 1 (slightly water-hazardous) AwSV.
7.2 Radioactivity
According to Geh2012 and RP 112 dose values and radon
concentrations of gypsum-based building products are below
0.3 mSv/a. Thus, they can be used without restrictions.
8 Environmental Product Declaration - Knauf Gips KG - Knauf Safeboard GKF
Name Value Unit VOC emission tests showed that Knauf Safeboard GKF
significantly undercuts the required thresholds.
TVOC ≤ 1.0 mg/m³
TSVOC ≤ 0.1 mg/m³
R-value (dimensionless) ≤ 1 -
Sum of VOC without NIK/LCI ≤ 0.1 mg/m³
Formaldehyde ≤ 0.1 mg/m³
Total carcinogens ≤ 0.001 mg/m³
8. References
Standards ISO 15686-1
ISO 15686-1:2011: Buildings and constructed assets -- Service
DIN 6812 life planning -- Part 1: General principles and framework
DIN 6812:2013-06, Medical X-ray equipment up to 300 kV -
Rules of construction for structural radiation protection ISO 45001
ISO 45001:2018, Occupational health and safety management
DIN 18180 systems – Requirements with guidance for use
DIN 18180:2014-09, Gypsum plasterboards - Types and
requirements ISO 50001
EN ISO 50001:2018, Energy management systems –
DIN 38404-5 Requirements with guidance for use
DIN 38404-5: 1984, German standard methods for the
examination of water, waste water and sludge; physical and Further References
physico-chemical parameters (group C); determination of the
pH-value (C 5) AwSV
Verordnung über Anlagen zum Umgang mit
EN 520 wassergefährdenden Stoffen 1,2 (AwSV) 18.04.2017 vom
EN 520:2009-12, Gypsum plasterboards - Definitions, Bundesministerium der Justiz
requirements and test methods
BBSR2017
EN 12664 Service life of building components for life cycle analyses acc.
DIN EN 12664: Thermal Performance of Building Materials and to the Sustainable Building Assessment System (BNB) --
Products - Determination of Thermal Resistance by Means of Nutzungsdauer von Bauteilen für Lebens-zyklusanalysen nach
Guarded Hot Plate and Heat Flow Meter Methods - Dry and Bewertungssystem Nachhaltiges Bauen (BNB) 2017-02-24 vom
Moist Products with Medium and Low Thermal Bundesinstitut für Bau-, Stadt-, Raumforschung (BBSR)
EN 13501-1 BDSH2013
Fire classification of construction products and building Bauschäden durch Hochwasser – Tipps für die Sanierung
elements – Part 1: Classification using data from reaction to fire (Flood damage - tips for recovery), instruction sheet, Knauf
tests; German version EN 13501-1:2018 Gips KG (editor), Iphofen, 2013, www.knauf.de
EN 15804 BG RCI
EN 15804:2012+A2:2019+AC:2021, Sustainability of Occupational health and safety management: Systematic
construction works — Environmental Product Declarations — Safety, editor: The German Social Accident Insurance
Core rules for the product category of construction products. Institution for the Raw Materials and Chemical Industry,
Heidelberg, 2021-12-01
ISO 9001
DIN EN ISO 9001:2015-09; Quality management system – BImSchG
Requirements Act on the Prevention of Harmful Effects on the Environment
Caused by Air Pollution, Noise, Vibration and Similar
ISO 10456 Phenomena (Federal Immission Control Act - BImSchG),
EN ISO 10456-1:2010-05: Building materials and products - Publication 2013-05-2017 (BGBI. I p. 1274), last amended
Hygrothermal properties – Tabulated design values and 2015-08-31 (BGBI. I p. 1474)
procedures for determining declared and design thermal
values - Technical Corrigendum 1 (ISO 10456:2007/Cor DepV
1:2009) Verordnung über Deponien und Langzeitlager
(Deponieverordnung – DepV), German landfill ordinance, last
ISO 11885 amended and supplemented: 2021-07-09
EN ISO 11885:2009, Water quality – Determination of selected
elements by inductively coupled plasma optical emission Dre2006
spectrometry (ICP-OES) H. Drexler, Test report no. 1080556 AU-23572, Dorfner
Analysenzentrum und Anlagenplanungsgesellschaft mbH,
ISO 14025 Hirschau, 11.01.2006 (originator: Bundesverband Gips e. V., Dr.
EN ISO 14025:2011, Environmental labels and declarations — H.-J. Kersten, Berlin)
Type III environmental declarations — Principles and
procedures. ECHA
European Chemicals Agency (ECHA), Candidate List of
Substances of Very High Concern for Authorisation (published
9 Environmental Product Declaration - Knauf Gips KG - Knauf Safeboard GKF
in accordance with Article 59(10) of the Regulation (EC) No 528/2012
REACH Regulation), http://echa.europa.eu/de/candidate-list- REGULATION (EU) No 528/2012 OF THE EUROPEAN
table, Revision: 2023-06-14 PARLIAMENT AND OF THE COUNCIL of 22 May 2012
concerning the making available on the market and use of
Eurofins2021 biocidal products
VOC Emission Test Report for Knauf Safeboard GKF 12.5 mm
by the institute 'Eurofins Product Testing A/S in Galten- Regulation (EC) No. 1272/2008
Denmark; 2021-02-23 REGULATION (EC) No 1272/2008 OF THE EUROPEAN
PARLIAMENT AND OF THE COUNCIL of 16 December 2008
European Waste Code on classification, labelling and packaging of substances and
Guidance on classification of waste according to EWC-Stat mixtures, amending and repealing Directives 67/548/EEC and
categories, Supplement to the Manual for the Implementation of 1999/45/EC, and amending Regulation (EC) No 1907/2006
the Regulation (EC) No 2150/2002 on Waste Statistics,
COMMISSION OF THE EUROPEAN RP112
COMMUNITIES/EUROSTAT, v2, December 2010 Radiation Protection 112: Radiological protection principles
concerning the natural radioactivity of building materials,
Geh2012 European Commission, Luxembourg, 2000
K. Gehrcke, B. Hoffmann, U. Schkade, V. Schmidt, K.
Wichterey: Natürliche Radioaktivität in Baumaterialien und die TRGS 521
daraus resultierende Strahlenexposition, Report BfS-SW-14/12, Technical Rules for Hazardous Substances TRGS 521:
Bundesamt für Strahlenschutz (editor), http://nbn- Demolition, reconstruction and maintenance work with
resolving.de/urn:nbn:de:0221-201210099810, Salzgitter, 2012 biopersistent mineral wools, Edition: February 2008, Federal
Institute for Occupational Safety and Health (editor)
Gips-DB
Gips-Datenbuch, editor: Bundesverband Gips e. V. (German TRGS 559
association of gypsum manufacturers), Berlin, 2013 Technical Rules for Hazardous Substances TRGS 559: Mineral
Dust, Edition: February 2010, Federal Institute for Occupational
IBU 2022 Safety and Health (editor), last amended and supplemented:
Institut Bauen und Umwelt e.V.: General Instructions for the GMBl 2011
EPD programme of Institut Bauen und Umwelt e.V., Version
2.1, Berlin: Institut Bauen und Umwelt e.V., 2022; www.ibu- TRGS 900
epd.com Technical Rules for Hazardous Substances TRGS 900:
Occupational Exposure Limits, Edition: January 2006, Federal
IBU PCR Part A Institute for Occupational Safety and Health (editor), last
Institut Bauen und Umwelt e.V.: Product Category Rules for amended and supplemented: GMBl 201
Building-Related Products and Services Part A: Calculation
Rules for the Life Cycle Assessment and Requirements on the Technical brochures Knauf
Project Report according to EN 15804+A2:2019, v1.1.2, Downloadable under www.knauf.de
2021-09-02
K11
IBU PCR Part B "Plasterboards" K11.de_ENG; Knauf X-ray Shielding Ceiling Systems, technical
Institut Bauen und Umwelt e.V.: PCR Guidance-Texts for document 2022-09
Building-Related Products and Services Part B: Requirements
on the EPD for Plasterboard, v5, 2023-07-11 K13
K13.de_ENG; Knauf X-ray Shielding Partitions, technical
LCA for Experts (GaBi) document 2022-09
LCA for Experts (v10.7.0.183): Software-System and
Databases for Life Cycle Engineering, Sphera Solutions GmbH, K15
Leinfelden- Echterdingen, Germany, 2023 (database version K15.de_ENG; Knauf X-ray Shielding Furring, technical
2023.1) document 2022-09
Regulation (EU) No 305/2011 K762
Regulation (EU) No 305/2011 for construction products (CPR), K762.de_ENG; Knauf Safeboard GKF; technical data sheet
Regulation (EU) No 305/2011 of the European Parliament and 2022-06
of the Council of 9 March 2011 laying down harmonized
conditions for the marketing of construction products ST02
ST02.de_ENG; Knauf Safeboard – X-ray Shielding, technical
brochure 2017-07
10 Environmental Product Declaration - Knauf Gips KG - Knauf Safeboard GKF
Publisher
Institut Bauen und Umwelt e.V. +49 (0)30 3087748- 0
Hegelplatz 1 info@ibu-epd.com
10117 Berlin www.ibu-epd.com
Germany
Programme holder
Institut Bauen und Umwelt e.V. +49 (0)30 3087748- 0
Hegelplatz 1 info@ibu-epd.com
10117 Berlin www.ibu-epd.com
Germany
Author of the Life Cycle Assessment
Knauf Gips KG 0049 9001 31-1000 *
Am Bahnhof 7 knauf-direkt@knauf.de
97346 Iphofen www.knauf.de
Germany
Owner of the Declaration
Knauf Gips KG 0049 9001 31-1000 *
Am Bahnhof 7 knauf-direkt@knauf.de
97346 Iphofen www.knauf.de
Germany
11 Environmental Product Declaration - Knauf Gips KG - Knauf Safeboard GKF
