ENVIRONMENTAL PRODUCT DECLARATION
as per ISO 14025 and EN 15804+A2
Owner of the Declaration Knauf Integral KG
Publisher Institut Bauen und Umwelt e.V. (IBU)
Programme holder Institut Bauen und Umwelt e.V. (IBU)
Declaration number EPD-KNA-20220094-CAB1-EN
Issue date 26.06.2023
Valid to 25.06.2028
Knauf GIFAfloor DB 36 green
Knauf Integral KG
www.ibu-epd.com | https://epd-online.com
General Information
Knauf Integral KG Knauf GIFAfloor DB 36 green
Programme holder Owner of the declaration
IBU – Institut Bauen und Umwelt e.V. Knauf Integral KG
Hegelplatz 1 Am Bahnhof 16
10117 Berlin 74589 Satteldorf
Germany Germany
Declaration number Declared product / declared unit
EPD-KNA-20220094-CAB1-EN 1 m² of gypsum fibre panel Knauf GIFAfloor DB 36 green, 57,9 kg/m², 36
mm
This declaration is based on the product category rules: Scope:
Plasterboard, 01.08.2021 This EPD declares the environmental impacts of the gypsum fibre panels
(PCR checked and approved by the SVR) Knauf GIFAfloor DB 36 green, produced by Knauf Integral KG, plant
Satteldorf (Germany). It covers 100 % of the manufacture of Knauf
GIFAfloor DB 36 green in Satteldorf (D). The life cycle assessment is
Issue date based on production data for 2020.
The owner of the declaration shall be liable for the underlying information
26.06.2023
and evidence; the IBU shall not be liable with respect to manufacturer
information, life cycle assessment data and evidences.
Valid to
The EPD was created according to the specifications of EN 15804+A2. In
25.06.2028 the following, the standard will be simplified as EN 15804.
Verification
The standard EN 15804 serves as the core PCR
Independent verification of the declaration and data according to ISO
14025:2011
internally X externally
Dipl.-Ing. Hans Peters
(Chairman of Institut Bauen und Umwelt e.V.)
Dipl.-Ing. Hans Peters Dr Naeem Adibi,
(Managing Director Institut Bauen und Umwelt e.V.) (Independent verifier)
1 Environmental Product Declaration - Knauf Integral KG - Knauf GIFAfloor DB 36 green
Product
or 1B (Regulation (EC) No. 1272/2008) which are not on the
Product description/Product definition candidate list, exceeding 0.1 percentage by mass: no
The declared product Knauf GIFAfloor DB 36 green is a
gypsum fibre board made of gypsum with paper fibres Biocide products were added to this construction product or it
suspended in the gypsum matrix for reinforcement of the has been treated with biocide products (this then concerns a
boards. The declared products have a thickness of 36 mm. treated product as defined by the (EU) Ordinance on Biocide
Further thicknesses (30 mm, 40 mm) are declared in separate Products No. 528/2012): no
EPDs. For the placing on the market of the product in the
European Union/European Free Trade Association (EU/EFTA) Reference service life
(with the exception of Switzerland) Regulation (EU) No reference service life according to ISO 15686 has been
No. 305/2011 (CPR) applies. The product needs a declaration determined for the declared products. However, a service life of
of performance taking into consideration EN 15283-2:2008 ≥ 50 years can be assumed for raised access floor panels
+ A1:2009, Gypsum boards with fibrous reinforcement - according to the BBSR table "Service lives of components for
Definitions, requirements and test methods - Part 2: Gypsum life cycle assessment according to BNB" (code no. 352.911).
fibre boards and the CE-marking. There are no influences on ageing when the panels are applied
in accordance with the rules of technology.
National provisions apply for the application and use.
Application Extraordinary effects
Knauf GIFAfloor DB green boards are used as raised access
floors panels with loose laid carpets or for access openings in Fire protection
dry hollow floor systems. Building material class A1
Applicable standards are: Burning droplets -
• EN 12825:2001, Raised access floors Smoke gas development -
• EN 13213:2001, Hollow floors
Contact with water
Technical Data Knauf GIFAfloor DB 36 green are designed to tolerate relative
Technical datasheets can be downloaded from the website humidities up to 75 %. Exceeding humidities or permanent
https://www.knauf-integral.de. exposure to wet conditions may lead to a decrease in strength
and should be avoided. However, due to the ingredients no
Constructional data of Knauf GIFAfloor DB 36 green
negative effect on human health is to be expected from
Name Value Unit
leaching.
Gross density acc. to EN 15283-2 ≥ 1500 kg/m3
Thermal conductivity acc. to EN ISO 10456 0.25 W/mK An instruction sheet about the restoration of flood damage is
available under www.knauf.de /BSDH/. Information about the
Calculation value for thermal conductivity 0.44 W/mK
removal of flood damage can also be downloaded from
Specific heat capacity 1 kJ/kgK
www.gypsum.org.
Water vapour diffusion resistance factor acc. to 10 - Due to the loose laying of Knauf GIFAfloor DB green panels
EN ISO 10456 affected panels can be easily replaced by new ones.
Water vapour diffusion resistance factor acc. to
4 -
EN ISO 10456 Re-use phase
0.5 - Knauf GIFAfloor DB 36 green panels are laid loosely on the
Moisture content at 20 °C, 65% humidity M.-%
0.9 sub-construction and is typically covered by self-laid loose
textile covering. Therefore, they can be removed without any
Elongation/Vibration when humidity changes by
≤ 1.00 mm/m damage to the panels and re-use is possible.
30% (20°C) acc. to EN 318
Performance data of the product in accordance with the According to the German Commercial Waste Ordinance
declaration of performance with respect to its essential GewAbfV construction and demolition based on gypsum is
characteristics according to EN 15283-2:2008 + A1:2009, preferably collected separately from other waste types and
Gypsum boards with fibrous reinforcement - Definitions, supplied to recycling facilities. In addition, Knauf GIFAfloor DB
requirements, and test methods - Part 2: Gypsum fibre boards. 36 green panels are designed to be easily recyclable.
Base materials/Ancillary materials
Disposal
Knauf GIFAfloor DB green panels consist of approx. 92 % w/w
Knauf GIFAfloor DB 36 green panels need to be dismanteled
set gypsum reinforced with > 7 % w/w paper fibres and < 0.5 %
and collected separately from other construction waste. If
additives. Knauf GIFAfloor DB green panels are impregnated
disposed, Knauf GIFAfloor DB 36 green panels need to be
with < 0.5 % w/w impregnating agent (surface impregnation).
disposed of as gypsum waste under the European Waste Code
(EWC)
The declared products contains substances listed in the
candidate list (date: 17.01.2023, ECHA) exceeding 0.1
17 08 02 - gypsum-based construction materials other than
percentage by mass: no.
those mentioned in 17 08 01
This product contains other CMR substances in categories 1A
LCA: Calculation rules
2 Environmental Product Declaration - Knauf Integral KG - Knauf GIFAfloor DB 36 green
with water leads to the re-incorporation of water of
Declared Unit crystallization into the crystal lattice of calcium sulphate. That
The declared unit is 1 m² of Knauf GIFAfloor DB 36 green way, gypsum becomes settled and hardened. Redundant
panels. The conversion factors and densities are given in the surface water is finally removed in a dryer.
table below:
Declared unit for Knauf GIFAfloor DB 36 green Cut-offs
Cut-off rules as required by EN 15804+A2 are respected. The
Name Value Unit
details are given in the background report. The environmental
Declared unit 1 m2 impacts imposed by these cut-offs are considered neglectable.
conversion factor [Mass/Declared Unit] to 1 kg 0.017 - In total, the cut off materials and processes are less than 5 % of
Grammage 57.9 kg/m2 the mass and energy flows in the modules (A1-A3).
Gross density ≥ 1500 kg/m3
Data quality
Layer thickness 0.036 m Datasets exclusively from GaBi databases (version 2022.1) are
The declared environmental impacts are average impacts for used for the LCA modelling. All datasets used have been
the production in plant Satteldorf. Water and energy updated in the last 5 years. For processes and materials, where
consumption is measured on an annual basis and allocated to no direct match is available, data from literature or expert
the various products by the annually produced surface area per judgements are applied. Only a few materials and processes
panel thickness. needed to be cut off due to missing information. Since these
cut-off materials and processes are only of small amounts (<< 1
Knauf Integral plant Satteldorf is specifically designed to % w/w), the total influence of these neglected inputs is
produce a fibre reinforced gypsum material called Knauf expected to be lower than 5 % of energy usage and mass.
GIFAtec which is adapted in shape, density, surface treatment,
and edge trimming to yield the desired products. Therefore, With respect to technological, geographic and time
results of the life cycle indicators are considered to be very representativeness, the overall data quality is evaluated to be
robust. 'satisfactory'.
The LCA was modeled with software GaBi and its Foreground data are related to production data from plant
corresponding databases (database version 2022.1). Satteldorf for the reference year 2020. Water and energy
consumption are monitored and reported on an annual basis
and allocated to the specific products based on annually
System boundary produced surface area per panel thickness. Since the
Type of the EPD: cradle to gate - with options, modules C1–C4, composition of the material is quite constant throughout the
and module D (A1–A3 + C+ D, additional modules: A4, A5) product range, the LCA results are considered to be quite
robust with respect to the foreground data.
This EPD includes the following life cycle stages:
Allocations
• provision of raw materials and transport to plant
Allocations in the foreground data have only been applied for
Satteldorf, production of boards (A1-A3) including
energy and water consumption data which is monitored on an
thermal energy for calcination and drying (from natural
annual basis for the whole production plant Satteldorf.
gas, geographic scope: DE), as well as electricity
Allocations in the background data are described and have not
(residual mix DE)
been adjusted.
• transport to building site (A4)
• installation at building site (A5) including the incineration
Paper fibres incorporated in the gypsum fibre panels are made
of transport packaging
from waste cardboard and enter the product system free of
• manual disassembly (C1)
burdens. Further allocations of production data have been
• transport to recycling facility or landfill site (C2)
avoided. However, there may be allocations in the background
• 2 scenarios for end of life:
data which are are explained in the documentation of the
• Scenario 1: landfilling (C4/1), corresponding to zero
respective datasets.
impacts in C3/1 and credits in D/1 from incineration of
packaging material in A5
Geographic Representativeness
• Scenario 2: recycling (C3/2), zero impacts in C4/2 and
Land or region, in which the declared product system is
credits for the recycled material beyond the system
manufactured, used or handled at the end of the product´s
boundaries and from A5 (D/2). Recycling includes the
lifespan: Global
electrical energy for the crushing and grinding of the
disassembled panels prior to backfeeding into the next
production cycle. Comparability
Basically, a comparison or an evaluation of EPD data is only
Fig. 1 illustrates the production process: Natural and Flue gas
possible if all the data sets to be compared were created
desulphurization (FGD) gypsum is calcined (removal of water of
according to EN 15804 and the building context, respectively
crystallization). The calcined stucco in mixed with additive and
the product-specific characteristics of performance, are taken
fibres from wastepaper and mixed with water. This slurry is fed
into account.
to an infinite belt with vacuum pumps. After this, the density of
the material is adjusted by a winding roller and a press. Mixing
3 Environmental Product Declaration - Knauf Integral KG - Knauf GIFAfloor DB 36 green
Fig. 1: Production process for gypsum fibre panels
LCA: Scenarios and additional technical information
freight ship are required for transportation. Due to these
Characteristic product properties of biogenic carbon different transportation vehicles employed, the transport
Information on describing the biogenic Carbon Content at distances for FGD gypsum were calculated with weighted
factory gate averages for a combined transportation by truck, river, and
ocean.
Name ValueUnit
kg
Biogenic carbon content in product 2.26 Further raw materials are supplied by truck from manufacturers
C
within Germany or from neighbouring countries.
Biogenic carbon content in accompanying kg
0.082
packaging C Manufacturing
Gypsum (natural and FGD gypsum) is calcined to stucco before
mixing with water. Stucco, cellulose fibres and small amounts of
Product Stage (A1-A3)
additives are then suspended in water to give a slurry . The
resulting mixture passes a job feeder and is fed on an infinite
Supply of raw materials
felt with vacuum pumps to remove excess water. Afterwards,
Knauf GIFAfloor DB green boards are gypsum fibre boards
the pulp is driven through a winding roller and a subsequent
consisting of gypsum with cellulose fibre from recycled
press for panel forming and further removal of water before it
cardboard incorporated in the gypsum matrix. Currently, natural
finally enters a dryer. Drying of surface moisture is followed by
gypsum from open-cast mining in close vicinity to the
surface finishing, formatting and edge processing as well as the
production plant as well as gypsum from the flue gas
application of the impregnating agent.
desulphurization of different coal fired power plants is used to
produce the boards.
(Transport) Packaging
Knauf GIFAfloor DB green panels are not packaged individually,
Small amounts of additives are used for easier processing and
but stacked on a wooden pallet (reusable), covered with a
fine adjustment of properties.
cardboard sheet and secured with PET straps.
Transport of raw materials
Natural gypsum is extracted from mines close to the Transport to the building site (A4)
manufacturing sites. Accordingly, transport distances are short As the default value, transportation over 500 km by truck was
(< 30 km) and trucks are used. FGD gypsum is transported by assumed for the transportation of the products to the building
truck from coal-fired power plants in Germany and Europe, site. This is no actual transport distance since transport
mainly. In few cases, a river freight ship and even an ocean distances can only be considered at the building level.
4 Environmental Product Declaration - Knauf Integral KG - Knauf GIFAfloor DB 36 green
Nevertheless, the provided numbers shall enable the A service life of ≥ 50 years can be assumed for raised access
calculation of the actual environmental burdens for the floor panels and ceiling and wall coverings according
transport of the declared products by inter-/extrapolating to the BBSR table "Service lives of components for life cycle
distances and mixing of transport means according to assessment according to BNB".
the conditions at hand for individual building assessments.
Hygrothermal in-use conditions (stationary): -10 °C to +35 °C;
However, since Knauf GIFAfloor DB green panels are shipped 35 to 75 % rel. air humidity
globally, further transportation scenarios were considered:
End of life (C1-C4)
- Scenario (A4/1): Transport by truck 1000 km
Knauf GIFAfloor DB 36 green are disassembled manually and
- Scenario (A4/2): Transport by rail 1000 km
collected separately from other deconstruction waste.
- Scenario (A4/3): Transport by ocean freight ship over 10000
Transportation in C2 is assumed to be 100 km by truck to either
km
an appropriate landfill site (scenario 1) or to a recycling facility
- Scenario (A4/4): Transport by river freight ship over 1000 km
(scenario 2).
The results of these further transportation scenarios are given
Since Knauf GIFAfloor DB 36 green are laid loosely, no
in the Annexe to this EPD.
adhering foreign material needs to be removed from the panels
prior to recycling (scenario 2). The panels are milled to fine
Default scenario (A4): Transport by truck 500 km
powder without any further material separation. The same
Name Value Unit energy consumption as for the milling of natural gypsum in
Litres of fuel 0.113 l/100km plant Satteldorf is assumed for the recycling procedure. The
Transport distance 500 km recycled gypsum is assumed to replace virgin FGD and natural
gypsum in the same ratio as it was initially introduced into
Capacity utilisation (including empty runs) 50 %
production cycle declared in modules A1-A3. No additional
Gross density of products transported ≥ 1500 kg/m3
processes are required for recycling.
Installation into the building (A5) Name ValueUnit
Raised access floor panels Knauf GIFAfloor DB green are Collected separately gypsum-based construction
57.9 kg
installed by being loosely laid on specific raised access floor materials
pedestals available at Knauf Integral KG according to Landfilling scenario 1 57.9 kg
the installation instructions. No sealing of joints is required. Recycling scenario 2 57.9 kg
Name Value Unit
With the definition of 2 end-of-life scenarios, benefits and loads
Electricity consumption - kWh beyond system boundaries are declared as follows:
Type of assembly manually D/1: contains only credits for exported energy from incineration
Construction waste 5 % of packaging material (results only from A5)
D/2: contains credits for exported energy from incineration of
Treatment of packaging
incineration packaging material in A5 and the benefits from the recycled
waste
material of Knauf GIFAfloor DB green panels replacing FGD
Components not Substructures, screws, jointing
and natural gypsum in the same ratio as both gypsum types
considered material
were introduced in A1-A3; amount of paper fibres is discounted
from weight of demolition waste to avoid double counting of
Use phase (B1-B7): Excluded since no environmental secondary material and replacement of gypsum by paper fibres.
impacts/benefits are expected.
5 Environmental Product Declaration - Knauf Integral KG - Knauf GIFAfloor DB 36 green
LCA: Results
Note: Two scenarios for the end of life stage were considered as 100 % scenario, each.
Scenario 1: Landfilling - module C4/1, C3/1 with zero impacts, D/1 (only from A5)
Scenario 2: Recycling - module C3/2, C4/2 with zero impacts, D/2 (from A5 and C3/2)
DESCRIPTION OF THE SYSTEM BOUNDARY (X = INCLUDED IN LCA; ND = MODULE OR INDICATOR NOT DECLARED; MNR =
MODULE NOT RELEVANT)
Benefits and
Construction loads beyond
Product stage Use stage End-of-life stage
process stage the system
boundaries
la ire ta m w a Ry lp p u s tro p s n a rT g n iru tc a fu n a M e h t m o rf tro p s n a rTe tis e h t o t e ta g y lb m e s s A e s U e c n a n e tn ia M ria p e R tn e m e c a lp e R tn e m h s ib ru fe R y g re n e la n o ita re p Oe s u re ta w la n o ita re p Oe s u n o itc u rts n o c -e Dn o itilo m e d tro p s n a rT g n is s e c o rp e ts a W la s o p s iD -e s u e R-y re v o c e R-g n ilc y c e Rla itn e to p
A1 A2 A3 A4 A5 B1 B2 B3 B4 B5 B6 B7 C1 C2 C3 C4 D
X X X X X MND MND MNR MNR MNR MND MND X X X X X
RESULTS OF THE LCA - ENVIRONMENTAL IMPACT according to EN 15804+A2: 1 m² Knauf GIFAfloor DB 36 green, 57.9 kg/m²,
36 mm
Parameter Unit A1-A3 A4 A5 C1 C2 C3/1 C3/2 C4/1 C4/2 D/1 D/2
GWP-total kg CO 2 eq 1.26E+00 2.05E+00 1.32E+00 0 4.13E-01 0 8.36E+00 9.43E+00 0 -1.08E-01 -8.6E+00
GWP-fossil kg CO 2 eq 9.84E+00 2.04E+00 6.85E-01 0 4.1E-01 0 5.97E-02 1.13E+00 0 -1.08E-01 -2.9E-01
GWP-
biogenic kg CO 2 eq -8.59E+00 0 6.31E-01 0 0 0 8.3E+00 8.3E+00 0 -5.51E-04 -8.31E+00
GWP-luluc kg CO 2 eq 1.91E-03 7.75E-03 7.02E-04 0 2.75E-03 0 1.26E-05 1.63E-03 0 -1.18E-05 -1.63E-04
kg CFC11
ODP 2.23E-11 4.64E-13 1.29E-12 0 5.04E-14 0 8.73E-13 2.32E-12 0 -7.28E-13 -1.3E-12
eq
AP mol H+ eq 3.22E-02 1.97E-03 2.14E-03 0 4.61E-04 0 1.31E-04 7.24E-03 0 -1.42E-04 -5.97E-04
EP-
kg P eq 2.95E-06 4.04E-06 2.26E-06 0 1.46E-06 0 1.74E-07 3.65E-05 0 -1.48E-07 -3.46E-07
freshwater
EP-marine kg N eq 9.37E-03 6.89E-04 6.47E-04 0 1.54E-04 0 2.94E-05 2.38E-03 0 -3.84E-05 -2.19E-04
EP-terrestrial mol N eq 1.04E-01 7.88E-03 7.01E-03 0 1.79E-03 0 3.08E-04 2.15E-02 0 -4.12E-04 -2.48E-03
kg NMVOC
POCP 2.61E-02 1.77E-03 1.84E-03 0 3.98E-04 0 7.94E-05 7.74E-03 0 -1.08E-04 -5.82E-04
eq
ADPE kg Sb eq 2.64E-06 2.04E-07 1.5E-07 0 4.15E-08 0 1.63E-08 1.04E-07 0 -1.63E-08 -3.29E-08
ADPF MJ 1.41E+02 2.7E+01 9.47E+00 0 5.4E+00 0 1.08E+00 1.49E+01 0 -1.83E+00 -3.86E+00
m3 world eq
WDP 5.66E-01 9.62E-03 6.94E-02 0 4.75E-03 0 1.36E-02 1.1E-01 0 -1.15E-02 -1.35E-02
deprived
GWP = Global warming potential; ODP = Depletion potential of the stratospheric ozone layer; AP = Acidification potential of land and water; EP =
Eutrophication potential; POCP = Formation potential of tropospheric ozone photochemical oxidants; ADPE = Abiotic depletion potential for non-fossil
resources; ADPF = Abiotic depletion potential for fossil resources; WDP = Water (user) deprivation potential)
RESULTS OF THE LCA - INDICATORS TO DESCRIBE RESOURCE USE according to EN 15804+A2: 1 m² Knauf GIFAfloor DB
36 green, 57.9 kg/m², 36 mm
Parameter Unit A1-A3 A4 A5 C1 C2 C3/1 C3/2 C4/1 C4/2 D/1 D/2
PERE MJ 4.25E+00 1.78E+00 7.28E+00 0 3.76E-01 0 7.67E+01 1.94E+00 0 -5.03E-01 -7.69E+01
PERM MJ 7.9E+01 0 -2.9E+00 0 0 0 -7.61E+01 0 0 0 7.61E+01
PERT MJ 8.32E+01 1.78E+00 4.38E+00 0 3.76E-01 0 6.01E-01 1.94E+00 0 -5.03E-01 -7.99E-01
PENRE MJ 1.41E+02 2.7E+01 9.56E+00 0 5.42E+00 0 1.08E+00 1.49E+01 0 -1.83E+00 -3.86E+00
PENRM MJ 8.85E-02 0 -8.85E-02 0 0 0 0 0 0 0 0
PENRT MJ 1.41E+02 2.7E+01 9.48E+00 0 5.42E+00 0 1.08E+00 1.49E+01 0 -1.83E+00 -3.86E+00
SM kg 4.41E+00 0 0 0 0 0 0 0 0 0 -5.35E+01
RSF MJ 0 0 0 0 0 0 0 0 0 0 0
NRSF MJ 0 0 0 0 0 0 0 0 0 0 0
FW m3 2.55E-02 1.42E-03 2.36E-03 0 4.39E-04 0 5.73E-04 3.31E-03 0 -4.84E-04 -8.36E-04
PERE = Use of renewable primary energy excluding renewable primary energy resources used as raw materials; PERM = Use of renewable primary
energy resources used as raw materials; PERT = Total use of renewable primary energy resources; PENRE = Use of non-renewable primary energy
excluding non-renewable primary energy resources used as raw materials; PENRM = Use of non-renewable primary energy resources used as raw
materials; PENRT = Total use of non-renewable primary energy resources; SM = Use of secondary material; RSF = Use of renewable secondary fuels;
NRSF = Use of non-renewable secondary fuels; FW = Use of net fresh water
RESULTS OF THE LCA – WASTE CATEGORIES AND OUTPUT FLOWS according to EN 15804+A2:
1 m² Knauf GIFAfloor DB 36 green, 57.9 kg/m², 36 mm
Parameter Unit A1-A3 A4 A5 C1 C2 C3/1 C3/2 C4/1 C4/2 D/1 D/2
HWD kg 2.38E-08 1.72E-10 1.27E-09 0 3.96E-11 0 9.37E-11 1.22E-09 0 -2.48E-10 -2.95E-10
NHWD kg 8.11E-02 4.45E-03 2.84E+00 0 8.95E-04 0 8.16E-04 5.68E+01 0 -9.26E-04 -1.73E-03
6 Environmental Product Declaration - Knauf Integral KG - Knauf GIFAfloor DB 36 green
RWD kg 5.95E-03 3.63E-05 3.12E-04 0 1.05E-05 0 1.73E-04 1.69E-04 0 -1.44E-04 -1.76E-04
CRU kg 0 0 0 0 0 0 0 0 0 0 0
MFR kg 0 0 0 0 0 0 5.79E+01 0 0 0 0
MER kg 0 0 0 0 0 0 0 0 0 0 0
EEE MJ 0 0 4.84E-01 0 0 0 0 0 0 0 0
EET MJ 0 0 8.71E-01 0 0 0 0 0 0 0 0
HWD = Hazardous waste disposed; NHWD = Non-hazardous waste disposed; RWD = Radioactive waste disposed; CRU = Components for re-use;
MFR = Materials for recycling; MER = Materials for energy recovery; EEE = Exported electrical energy; EET = Exported thermal energy
RESULTS OF THE LCA – additional impact categories according to EN 15804+A2-optional:
1 m² Knauf GIFAfloor DB 36 green, 57.9 kg/m², 36 mm
Parameter Unit A1-A3 A4 A5 C1 C2 C3/1 C3/2 C4/1 C4/2 D/1 D/2
Disease
PM 9.51E-07 1.26E-08 5.29E-08 0 3.16E-09 0 1.09E-09 8.47E-08 0 -1.17E-09 -4.16E-07
incidence
IR kBq U235 eq 4.69E-01 3.69E-03 2.54E-02 0 1.56E-03 0 2.93E-02 2.05E-02 0 -2.44E-02 -2.76E-02
ETP-fw CTUe 5.29E+01 2.05E+01 4.4E+00 0 3.81E+00 0 4.74E-01 1.01E+01 0 -4.02E-01 -1.14E+00
HTP-c CTUh 1.53E-09 4.11E-10 1.57E-10 0 7.85E-11 0 1.36E-11 1.08E-09 0 -1.85E-11 -3.63E-11
HTP-nc CTUh 1.28E-07 2.08E-08 1.39E-08 0 4.26E-09 0 4.98E-10 1.22E-07 0 -7.1E-10 -1.8E-09
SQP SQP 4.96E+01 8.02E+00 3.14E+00 0 2.27E+00 0 3.9E-01 2.59E+00 0 -3.27E-01 -9.7E-01
PM = Potential incidence of disease due to PM emissions; IR = Potential Human exposure efficiency relative to U235; ETP-fw = Potential comparative
Toxic Unit for ecosystems; HTP-c = Potential comparative Toxic Unit for humans (cancerogenic); HTP-nc = Potential comparative Toxic Unit for humans
(not cancerogenic); SQP = Potential soil quality index
Disclaimer 1 – for the indicator “Potential Human exposure efficiency relative to U235”. This impact category deals mainly with the
eventual impact of low dose ionizing radiation on human health of the nuclear fuel cycle. It does not consider effects due to possible
nuclear accidents, occupational exposure nor due to radioactive waste disposal in underground facilities. Potential ionizing radiation
from the soil, from radon and from some construction materials is also not measured by this indicator.
Disclaimer 2 – for the indicators “abiotic depletion potential for non-fossil resources”, “abiotic depletion potential for fossil resources”,
“water (user) deprivation potential, deprivation-weighted water consumption”, “potential comparative toxic unit for ecosystems”,
“potential comparative toxic unit for humans – cancerogenic”, “Potential comparative toxic unit for humans - not cancerogenic”,
“potential soil quality index”. The results of this environmental impact indicator shall be used with care as the uncertainties on these
results are high or as there is limited experienced with the indicator.
References
Standards ISO 14025
DIN EN ISO 14025:2011-10, Environmental labels
and declarations — Type III environmental declarations
EN 318 — Principles and procedures.
EN 318:2002-06 Wood-based panels - Determination of
dimensional changes associated with changes in relative ISO 14040
humidity ISO 14040:2006 + Amd 1:2020, Environmental management –
Life cycle assessment – Principles and framework
EN ISO 10456
EN ISO 10456:2010-05, Building materials and products - ISO 14044
Hygrothermal properties - Tabulated design values ISO 14044:2006 + Amd 1:2017 + Amd 2:2020,
and procedures for determining declared and design thermal Environmental management – Life cycle assessment –
values (ISO 10456:2007 + Cor. 1:2009) Requirements and guidelines
EN 12825 ISO 15686
EN 12825:2001, Raised access floors ISO 15686-2:2012-05, Buildings and constructed assets -
Service life planning - Part 2: Service life prediction procedures
EN 13213
EN 13213:2001, Hollow floors Further References
EN 13501 BBSR
EN 13501-1: 2018, Fire classification of construction products table "Service lives of components for life cycle
and building elements - Part 1: Classification using data from assessment according to BNB"
reaction to fire tests http://www.nachhaltigesbauen.de/baustoffund-
gebaeudedaten/nutzungsdauern-von-bauteilen.html, published
EN 15283 2017, last accessed 2022-09-29
EN 15283-2:2008 + A1:2009, Gypsum boards with fibrous
reinforcement - Definitions, requirements, and test methods - ECHA
Part 2: Gypsum fibre boards European Chemicals Agency (ECHA), Candidate List
of Substances of Very High Concern for Authorisation
EN 15804 (published in
EN 15804:2019+A2, Sustainability of construction works accordance with Article 59(10) of the REACH
— Environmental Product Declarations — Core rules for Regulation) http://echa.europa.eu/de/candidate-list-table,
the product category of construction products. Revision: 2023-
01-17
7 Environmental Product Declaration - Knauf Integral KG - Knauf GIFAfloor DB 36 green
for Building-Related Products and Services Part A:
European Waste Code Calculation Rules for the Life Cycle Assessment and
Guidance on classification of waste according to EWC- Requirements on the Project Report according to EN
Stat categories, Supplement to the Manual for the 15804+A2:2019, v1.1.2, 2021-09-02
Implementation of the Regulation (EC) No 2150/2002 on Waste
Statistics, COMMISSION OF THE IBU PCR Part B "Plasterboards"
EUROPEAN COMMUNITIES/EUROSTAT, v2, December 2010 Institut Bauen und Umwelt e.V.: PCR Guidance-Texts
for Building-Related Products and Services Part B:
GaBi Requirements on the EPD for Plasterboard, v1.7, 2019-01-04
GaBi ts (v10.6.1.35): Software-System and Databases for
Life Cycle Engineering, Sphera Solutions GmbH, Leinfelden- (EU) Ordinance on Biocide Products No. 528/2012
Echterdingen, Germany, 2022 (database version 2022.1) REGULATION (EU) No 528/2012 OF THE
EUROPEAN PARLIAMENT AND OF THE COUNCIL of 22 May
GewAbfV 2012 concerning the making available on the market and use
Verordnung über die Bewirtschaftung von of biocidal products
gewerblichen Siedlungsabfällen und von bestimmten Bau-
und Abbruchabfällen (Gewerbeabfallverordnung - GewAbfV) Regulation (EU) No. 305/2011
Gewerbeabfallverordnung vom 18. April 2017 (BGBl. I S. 896), REGULATION (EU) No 305/2011 OF THE
last amended by Artikel 3 der Verordnung vom 28. April 2022 EUROPEAN PARLIAMENT AND OF THE COUNCIL of 9 March
(BGBl. I S. 700) 2011 laying down harmonised conditions for the marketing
German Commercial Waste Ordinance of construction products and repealing Council
Directive 89/106/EEC
IBU 2021
Institut Bauen und Umwelt e.V.: Allgemeine Anleitung für Regulation (EC) No. 1272/2008
das EPD-Programm des Institut Bauen und Umwelt e.V. REGULATION (EC) No 1272/2008 OF THE
(IBU). Version 2.0, Berlin: Institut Bauen und Umwelt e.V., EUROPEAN PARLIAMENT AND OF THE COUNCIL of 16
2021. December 2008 on classification, labelling and packaging of
www.ibu-epd.com substances and mixtures, amending and repealing Directives
67/548/EEC
IBU PCR Part A and 1999/45/EC, and amending Regulation (EC) No 1907/2006
Institut Bauen und Umwelt e.V.: Product Category Rules
8 Environmental Product Declaration - Knauf Integral KG - Knauf GIFAfloor DB 36 green
Publisher
Institut Bauen und Umwelt e.V. +49 (0)30 3087748- 0
Hegelplatz 1 info@ibu-epd.com
10117 Berlin www.ibu-epd.com
Germany
Programme holder
Institut Bauen und Umwelt e.V. +49 (0)30 3087748- 0
Hegelplatz 1 info@ibu-epd.com
10117 Berlin www.ibu-epd.com
Germany
Author of the Life Cycle Assessment
Knauf Gips KG 0049 9001 31-1000 *
Am Bahnhof 7 knauf-direkt@knauf.de
97346 Iphofen www.knauf.de
Germany
Owner of the Declaration
Knauf Integral KG +49 (7951) 497-0
Am Bahnhof 16 info@knauf-integral.de
74589 Satteldorf https://www.knauf-integral.de/de/
Germany
9 Environmental Product Declaration - Knauf Integral KG - Knauf GIFAfloor DB 36 green
