ENVIRONMENTAL PRODUCT DECLARATION
as per ISO 14025 and EN 15804+A2
Owner of the Declaration Kingspan Insulation B.V.
Publisher Institut Bauen und Umwelt e.V. (IBU)
Programme holder Institut Bauen und Umwelt e.V. (IBU)
Declaration number EPD-KSI-20230322-CBA2-EN
Issue date 22.09.2023
Valid to 21.09.2028
Kooltherm® K3 / Kooltherm® K10
Kingspan Insulation B.V.
www.ibu-epd.com | https://epd-online.com
General Information
Kingspan Insulation B.V. Kooltherm® K3 / Kooltherm® K10
Programme holder Owner of the declaration
IBU – Institut Bauen und Umwelt e.V. Kingspan Insulation B.V.
Hegelplatz 1 Lingewei 8
10117 Berlin 4004LL Tiel
Germany Netherlands
Declaration number Declared product / declared unit
EPD-KSI-20230322-CBA2-EN Kooltherm® K3 Floor Board / Kooltherm® K10 Soffit Board
1 m², 80 mm thickness, R = 3,80 m²·K/W
D
This declaration is based on the product category rules: Scope:
Insulating materials made of foam plastics, 01.08.2021 The insulation material Kooltherm® K3 / Kooltherm® K10 is produced by
(PCR checked and approved by the SVR) Kingspan Insulation B.V. at the manufacturing facilities in Tiel, the
Netherlands and Jönköping, Sweden. This EPD is based on weighted
averages which have been determined on the basis of the single values
Issue date originating from the different Kingspan Insulation factories.
22.09.2023
Kooltherm® K3 / Kooltherm® K10 is a rigid thermoset cellular insulation
material faced on both sides with a glass tissue based facing.
Valid to
In order to enable the user of the EPD to calculate the LCA results for
21.09.2028 different thicknesses, the EPD contains the respective calculation rules.
The owner of the declaration shall be liable for the underlying information
and evidence; the IBU shall not be liable with respect to manufacturer
information, life cycle assessment data and evidences.
The EPD was created according to the specifications of EN 15804+A2. In
the following, the standard will be simplified as EN 15804.
Verification
The standard EN 15804 serves as the core PCR
Dipl.-Ing. Hans Peters Independent verification of the declaration and data according to ISO
(Chairman of Institut Bauen und Umwelt e.V.) 14025:2011
internally X externally
Florian Pronold Vito D'Incognito,
(Managing Director Institut Bauen und Umwelt e.V.) (Independent verifier)
1 Environmental Product Declaration - Kingspan Insulation B.V. - Kooltherm® K3 / Kooltherm® K10
Product
Performance data of the product in accordance with the
Product description/Product definition declaration of performance with respect to its essential
Kooltherm® K3 / Kooltherm® K10 is a rigid thermoset cellular characteristics according to EN 13166 - Thermal insulation
insulation material faced on both sides with a glass tissue products for buildings - Factory made phenolic foam (PF)
based facing. The product is available in variable thicknesses products - Specification
from 20 mm up to 160 mm. This EPD is based on a thickness
of 80 mm and R -value of 3,80 m²·K/W. Base materials/Ancillary materials
D
The main materials are phenolic (PF) resin (between 70-80%)
with added catalyst and additives (between 15-20%). Phenolic
For the placing on the market of the product in the European
rigid foam onto a facing material (between 5-10%) is formed by
Union/European Free Trade Association (EU/EFTA) (with the
the chemical reaction of these materials and adding a blowing
exception of Switzerland) Regulation (EU) No. 305/2011 (CPR)
agent with no ozone depletion potential (ca. 5%). Due to the
applies. The product needs a declaration of performance taking
closed-cell structure (conform EN 13166), the blowing agent
into consideration EN 13166 - Thermal insulation products for
remains in the foam.
buildings - Factory made phenolic foam (PF) products -
specification and the CE-marking. For the application and use
In the current REACH regulations, phenolic foam insulation
the respective national provisions apply.
products are considered 'articles' and are exempt from the
Application requirements of Article 57 and 59(1) of REACH Regulation (EC)
Kooltherm® K3 is suitable for use as floor insulation. No 1907/2006. These products are not classified as 'hazardous
Kooltherm® K10 is suitable for use as soffit insulation. products' according to any current legislation, and can hence
be declared as follows:
Technical Data - This article contains substances listed in the candidate list
The declaration of performance of the product can be found at (date: 17.01.2023) exceeding 0.1 percentage by mass: no.
www.kingspan.com. - This article contains other carcinogenic, mutagenic, reprotoxic
(CMR) substances in categories 1A or 1B which are not on the
Constructional data
candidate list, exceeding 0.1 percentage by mass: no.
Name Value Unit - Biocide products were added to this construction product, or it
Compressive strength acc. to EN 13166 ≥ 100 kPa has been treated with biocide products (this then concerns a
Tensile strength perpendicular to faces acc. to treated product as defined by the (EU) Biocidal Products
≥ 60 kPa
EN 13166 Regulation No. 528/2012 (BPR): no.
Thermal conductivity λd acc. to EN 13166 for d
0.021W/(mK) The chemical functional group of the additives used in the resin
= 20 – 160 mm
is that of non-ionic surfactants.
Thermal conductivity λd acc. to EN 13166 for d
0.021W/(mK)
= 160 – 200 mm (2 layers) Reference service life
Technical parameters not included are modulus of elasticity as The reference service life is not to be declared in this EPD as it
well as sound absorption (not relevant for this application) and does not cover the use stage.
creep (not placed under permanent load). See Declaration of
Performance for further information.
LCA: Calculation rules
Multiplication factors are included to calculate impacts for other
Declared Unit product thicknesses within the range of 20 to 160 mm.
The declared unit (1 m²) and conversion factors are listed in the
table below. System boundary
The type of EPD according to EN 15804 is: cradle to gate with
Declared unit
options, modules C1–C4, and module D (A1–A3, C, D and
Name Value Unit
additional modules:A4, A5).
Declared unit 1 m2
Gross density (foam) 35 kg/m3 The product stage is a mandatory information module and it
Grammage 2.94 kg/m2 covers:
· A1, raw material extraction and processing, processing of
Layer thickness 0.08 m
secondary material input (e.g. recycling processes),
This EPD is based on a weighted average of the annual · A2, transport to the manufacturer,
production volume of two factories producing the products · A3, manufacturing, including provision of all materials,
Kooltherm® K3 / Kooltherm® K10. The scope of this EPD is the products and energy, packaging processing and its transport,
thermal insulation product Kooltherm® K3 / Kooltherm® K10 as as well as waste processing up to the end-of-waste state or
produced by Kingspan Insulation at the manufacturing facilities disposal of final residues during the product stage.
in Tiel (the Netherlands), Jönköping (Sweden). The
environmental impacts have been calculated per plant over the The construction process stage includes:
calendar year 2022. Based on the one-year production volume · A4 transport to the building site;
of Kooltherm® K3 / Kooltherm® K10 per plant, the individual · A5 installation in the building including provision of all
materials, products and energy, as well as waste processing up
environmental impacts are weighted.
to the end-of-waste state or disposal of final residues during the
construction process stage.
The EPD is studied for a common product thickness of 80mm.
The end-of-life stage is a mandatory information module and it
2 Environmental Product Declaration - Kingspan Insulation B.V. - Kooltherm® K3 / Kooltherm® K10
covers:
· C1 de-construction, demolition; Environmental burden of the incineration (R1 > 60 %) of the
· C2 transport to waste processing; product at the end-of-life stage are assigned to the product
· C3 waste processing for reuse, recovery and/or recycling; system(C3); resulting potential credits for thermal and electrical
· C4 disposal (not applicable for this EPD) including provision energy from energy substitution are declared in module D.
and all transport, provision of all materials, products and related
energy and water use.
Factors for different thicknesses Geographic Representativeness
The LCA results for the insulation material declared in this EPD Land or region, in which the declared product system is
refer to a product with a thickness of 80 mm. To enable the user manufactured, used or handled at the end of the product´s
of the EPD to calculate the results for different thicknesses the lifespan: Europe
factors in the following table can be used for the calculation.
The LCA results in chapter 5 have to be multiplied by these
Comparability
factors. The scaling factors are applicable for the complete
Basically, a comparison or an evaluation of EPD data is only
product, where the facings are for all product thicknesses
possible if all the data sets to be compared were created
equal, and the foam inputs are scaling upwards and
according to EN 15804 and the building context, respectively
downwards with other product thicknesses.
the product-specific characteristics of performance, are taken
into account.
Background data from GaBi ts Version 10 is used with GaBi
data sets CUP2022.1
LCA: Scenarios and additional technical information
Characteristic product properties of biogenic carbon
The total mass of biogenic carbon containing materials is less
than 5 % of the total mass of the product and accompanying
Installation into the building (A5)
packaging.
Note: 1 kg of biogenic carbon is equivalent to 44/12 kg of CO . Name ValueUnit
2
Output substances following waste treatment on
0.06 kg
site packaging material
Technical information The recycling of the packaging is considered in A5.
The following technical information is a basis for the declared
modules or can be used for developing specific scenarios in the
End of life (C1-C4)
context of a building assessment.
The assumptions for C1 are: diesel driven excavator (100 kW;
0.2 litre fuel per ton excavated material).
Manufacturing (A3)
The assumptions for C2 are: Truck Euro 6, diesel driven, 26-28
Within A1-A3 the following packaging of the final product is
t gross weight, assumed distance 50 km
included:
Polyethylene cover and wrap: 0,05 kg/m² Name Value Unit
Others (mainly Expanded Polystyrene skid): 0,01 kg/m² Collected as mixed construction waste 2.94 kg
Energy recovery 2.94 kg
Transport to the building site (A4) R1-value of waste incineration plant >60 %
Name Value Unit
Litres of fuel 0.0103 l/100km Reuse, recovery and/or recycling potentials (D),
Transport distance 100 km relevant scenario information
Grammage of products transported 2,94 kg/m²
Waste incineration with energy recuperation is assumed as
end-of-life scenario.
3 Environmental Product Declaration - Kingspan Insulation B.V. - Kooltherm® K3 / Kooltherm® K10
LCA: Results
DESCRIPTION OF THE SYSTEM BOUNDARY (X = INCLUDED IN LCA; MND = MODULE OR INDICATOR NOT DECLARED; MNR
= MODULE NOT RELEVANT)
Benefits and
Construction loads beyond
Product stage Use stage End of life stage
process stage the system
boundaries
la ire ta m w a Ry lp p u s tro p s n a rT g n iru tc a fu n a M e h t m o rf tro p s n a rTe tis e h t o t e ta g y lb m e s s A e s U e c n a n e tn ia M ria p e R tn e m e c a lp e R tn e m h s ib ru fe R y g re n e la n o ita re p Oe s u re ta w la n o ita re p Oe s u n o itc u rts n o c -e Dn o itilo m e d tro p s n a rT g n is s e c o rp e ts a W la s o p s iD -e s u e R-y re v o c e R-g n ilc y c e Rla itn e to p
A1 A2 A3 A4 A5 B1 B2 B3 B4 B5 B6 B7 C1 C2 C3 C4 D
X X X X X MND MND MNR MNR MNR MND MND X X X X X
RESULTS OF THE LCA - ENVIRONMENTAL IMPACT according to EN 15804+A2: 1 m2 80 mm thickness
Parameter Unit A1-A3 A4 A5 C1 C2 C3 C4 D
GWP-total kg CO 2 eq 5.56E+00 2.47E-02 1.5E-01 1.89E-03 1.24E-02 6.43E+00 0 -2.54E+00
GWP-fossil kg CO 2 eq 5.54E+00 2.46E-02 1.5E-01 1.88E-03 1.23E-02 6.43E+00 0 -2.52E+00
GWP-biogenic kg CO 2 eq -3.84E-02 -3.41E-05 8.17E-06 2.52E-06 -1.7E-05 4.37E-04 0 -1.29E-02
GWP-luluc kg CO 2 eq 6.38E-02 1.37E-04 1.77E-06 2.32E-08 6.87E-05 1.14E-05 0 -2.78E-04
ODP kg CFC11 eq 1.14E-08 1.48E-15 2.66E-14 1.16E-16 7.39E-16 4.7E-13 0 -1.71E-11
AP mol H+ eq 1.13E-02 2.54E-05 1.86E-05 8.75E-06 1.27E-05 3.79E-03 0 -3.33E-03
EP-freshwater kg P eq 1.87E-05 7.36E-08 6.73E-09 3.8E-10 3.68E-08 1.27E-07 0 -3.48E-06
EP-marine kg N eq 3.18E-03 8.31E-06 5E-06 4.17E-06 4.16E-06 1.84E-03 0 -9.01E-04
EP-terrestrial mol N eq 3.16E-02 9.89E-05 8.48E-05 4.57E-05 4.95E-05 2.11E-02 0 -9.65E-03
kg NMVOC
POCP 1.66E-02 2.24E-05 1.44E-05 1.18E-05 1.12E-05 4.71E-03 0 -2.52E-03
eq
ADPE kg Sb eq 5.76E-06 2.06E-09 6.5E-10 7.71E-11 1.03E-09 1.3E-08 0 -3.82E-07
ADPF MJ 1.61E+02 3.29E-01 5.52E-02 2.55E-02 1.65E-01 1.66E+00 0 -4.29E+01
m3 world eq
WDP 8.79E-01 2.21E-04 1.42E-02 3.5E-06 1.11E-04 6.33E-01 0 -2.7E-01
deprived
GWP = Global warming potential; ODP = Depletion potential of the stratospheric ozone layer; AP = Acidification potential of land and water; EP =
Eutrophication potential; POCP = Formation potential of tropospheric ozone photochemical oxidants; ADPE = Abiotic depletion potential for non-fossil
resources; ADPF = Abiotic depletion potential for fossil resources; WDP = Water (user) deprivation potential)
RESULTS OF THE LCA - INDICATORS TO DESCRIBE RESOURCE USE according to EN 15804+A2: 1 m2 80 mm thickness
Parameter Unit A1-A3 A4 A5 C1 C2 C3 C4 D
PERE MJ 2.06E+01 1.87E-02 1.42E-02 9.63E-05 9.36E-03 2.89E-01 0 -1.18E+01
PERM MJ 0 0 0 0 0 0 0 0
PERT MJ 2.06E+01 1.87E-02 1.42E-02 9.63E-05 9.36E-03 2.89E-01 0 -1.18E+01
PENRE MJ 7.88E+01 3.3E-01 2.6E+00 2.55E-02 1.65E-01 8.19E+01 0 -4.29E+01
PENRM MJ 8.27E+01 0 -2.55E+00 0 0 -8.02E+01 0 0
PENRT MJ 1.62E+02 3.3E-01 5.53E-02 2.55E-02 1.65E-01 1.66E+00 0 -4.29E+01
SM kg 0 0 0 0 0 0 0 0
RSF MJ 0 0 0 0 0 0 0 0
NRSF MJ 0 0 0 0 0 0 0 0
FW m3 3.5E-02 2.12E-05 3.37E-04 1.45E-07 1.06E-05 1.49E-02 0 -1.14E-02
PERE = Use of renewable primary energy excluding renewable primary energy resources used as raw materials; PERM = Use of renewable primary
energy resources used as raw materials; PERT = Total use of renewable primary energy resources; PENRE = Use of non-renewable primary energy
excluding non-renewable primary energy resources used as raw materials; PENRM = Use of non-renewable primary energy resources used as raw
materials; PENRT = Total use of non-renewable primary energy resources; SM = Use of secondary material; RSF = Use of renewable secondary fuels;
NRSF = Use of non-renewable secondary fuels; FW = Use of net fresh water
RESULTS OF THE LCA – WASTE CATEGORIES AND OUTPUT FLOWS according to EN 15804+A2:
1 m2 80 mm thickness
Parameter Unit A1-A3 A4 A5 C1 C2 C3 C4 D
HWD kg 7.65E-05 1.58E-12 4.6E-12 8.44E-14 7.91E-13 2.29E-10 0 -5.81E-09
NHWD kg 8.67E-02 4.73E-05 1.34E-02 2.39E-06 2.37E-05 3.23E-02 0 -2.17E-02
RWD kg 1.84E-03 4.07E-07 2.3E-06 2.8E-08 2.03E-07 6.85E-05 0 -3.39E-03
CRU kg 0 0 0 0 0 0 0 0
MFR kg 0 0 0 0 0 0 0 0
MER kg 0 0 5.99E-02 0 0 2.91E+00 0 0
EEE MJ 0 0 2.72E-01 0 0 1.11E+01 0 0
EET MJ 0 0 4.86E-01 0 0 1.99E+01 0 0
HWD = Hazardous waste disposed; NHWD = Non-hazardous waste disposed; RWD = Radioactive waste disposed; CRU = Components for re-use;
MFR = Materials for recycling; MER = Materials for energy recovery; EEE = Exported electrical energy; EET = Exported thermal energy
4 Environmental Product Declaration - Kingspan Insulation B.V. - Kooltherm® K3 / Kooltherm® K10
RESULTS OF THE LCA – additional impact categories according to EN 15804+A2-optional:
1 m2 80 mm thickness
Parameter Unit A1-A3 A4 A5 C1 C2 C3 C4 D
Disease
PM 1.16E-07 1.47E-10 2.27E-10 9.91E-11 7.33E-11 1.05E-08 0 -2.75E-08
incidence
IR kBq U235 eq 2.83E-01 5.96E-05 3.16E-04 4.08E-06 2.98E-05 1.1E-02 0 -5.74E-01
ETP-fw CTUe 5.98E+01 2.29E-01 3.95E-02 1.77E-02 1.14E-01 5.66E-01 0 -9.45E+00
HTP-c CTUh 2.73E-09 4.61E-12 2.22E-12 3.28E-13 2.31E-12 4.28E-11 0 -4.33E-10
HTP-nc CTUh 8.59E-08 2.39E-10 2.24E-10 1.66E-11 1.2E-10 1.55E-09 0 -1.66E-08
SQP SQP 1.08E+01 1.13E-01 1.41E-02 7.03E-05 5.67E-02 3.47E-01 0 -7.68E+00
PM = Potential incidence of disease due to PM emissions; IR = Potential Human exposure efficiency relative to U235; ETP-fw = Potential comparative
Toxic Unit for ecosystems; HTP-c = Potential comparative Toxic Unit for humans (cancerogenic); HTP-nc = Potential comparative Toxic Unit for humans
(not cancerogenic); SQP = Potential soil quality index
Disclaimer 1 – for the indicator “Potential Human exposure efficiency relative to U235”. This impact category deals mainly with the
eventual impact of low-dose ionizing radiation on human health of the nuclear fuel cycle. It does not consider effects due to possible
nuclear accidents, occupational exposure or radioactive waste disposal in underground facilities. Potential ionizing radiation from the
soil, radon and from some construction materials is also not measured by this indicator.
Disclaimer 2 – for the indicators “abiotic depletion potential for non-fossil resources”, “abiotic depletion potential for fossil resources”,
“water (user) deprivation potential, deprivation-weighted water consumption”, “potential comparative toxic unit for ecosystems”,
“potential comparative toxic unit for humans – cancerogenic”, “Potential comparative toxic unit for humans - not cancerogenic”,
“potential soil quality index”. The results of this environmental impact indicator shall be used with care as the uncertainties on these
results are high as there is limited experience with the indicator.
This EPD was created using a software tool.
References
EN 13166 ISO 14025
EN 13166:2012+A2:2016: Thermal insulation products EN ISO 14025:2011-10 - Environmental labels and declarations
for buildings. Factory made phenolic foam (PF) — Type III environmental declarations — Principles and
products. Specification procedures
EN 15804 LCA-tool
EN 15804:2012+A2:2019+AC:2021, Sustainability of Kingspan LCA tool, version 1.2. IBU-KSI-202001-LT1-EN.
construction works — Environmental Product Declarations — Developed by Sphera Solutions GmbH (formely Thinkstep
Core rules for the product category of construction products. GmbH)
BPR PCR Version 1.7, Part A
Regulation (EU) No 528/2012 of the European Parliament and Institut Bauen und Umwelt e.V., Berlin (pub.): Product Category
of the Council of 22 May 2012 concerning the making available Rules for Building-Related Products andservices, Part A:
on the market and use of biocidal products Calculation Rules for the Life Cycle Assessment and
Requirements on the Project Report according to EN
15804+A2:2019 November 2021
CPR
Regulation (EU) No. 305/2011 of the European Parliament and
of the Council of 9 March 2011 laying down harmonised PCR, Part B
condition for the marketing of construction products and Institut Bauen und Umwelt e.V., Berlin (pub.): Product Category
repealing Council Directive89/106/EC Rules for Construction Products from the range of
Environmental Product Declarations of Institut Bauen und
Umwelt (IBU), Part B: Requirements on the EPD for insulating
GaBi ts materials made of foam plastics. June 2023
thinkstep AG: Leinfelden-Echterdingen GaBi Software- System
and Database for Life Cycle Engineering 1992-2019
REACH
Regulation (EC) No 1907/2006 of the European Parliament and
IBU 2021 of the Council on the Registration, Evaluation, Authorisation
Institut Bauen und Umwelt e.V.: General Instructions for the and Restriction of Chemicals (REACH)
EPD programme of Institut Bauen und Umwelte.V., Version 2.0, https://echa.europa.eu/candidate-list-table; accessed 17th of
Berlin: Institut Bauen und Umwelte.V., 2021. www.ibu-epd.com January 2023, 233 substances listed.
5 Environmental Product Declaration - Kingspan Insulation B.V. - Kooltherm® K3 / Kooltherm® K10
Publisher
Institut Bauen und Umwelt e.V. +49 (0)30 3087748- 0
Hegelplatz 1 info@ibu-epd.com
10117 Berlin www.ibu-epd.com
Germany
Programme holder
Institut Bauen und Umwelt e.V. +49 (0)30 3087748- 0
Hegelplatz 1 info@ibu-epd.com
10117 Berlin www.ibu-epd.com
Germany
Author of the Life Cycle Assessment
Kingspan Insulation B.V. +31 (0) 543 543 210
Lingewei 8 info@kingspaninsulation.nl
4004LL Tiel www.kingspan.com
Netherlands
Owner of the Declaration
Kingspan Insulation B.V. +31 (0) 543 543 210
Lingewei 8 info@kingspaninsulation.nl
4004LL Tiel www.kingspan.com
Netherlands
6 Environmental Product Declaration - Kingspan Insulation B.V. - Kooltherm® K3 / Kooltherm® K10
