Environmental product declaration
In accordance with 14025 and EN15804+A2
Leca® Uno, Leca Portugal
Owner of the declaration: Program operator:
Leca International The Norwegian EPD Foundation
Product: Declaration number:
Leca® Uno, Leca Portugal
Registration number:
Declared unit:
1 m3 Issue date:
This declaration is based on Product Category Rules: Valid to:
CEN Standard EN 15804:2012+A2:2019 serves as core
EPD Software:
PCR
The Norwegian EPD Foundation LCA.no EPD generator ID: 57937
NPCR Part A: Construction products and services. Ver.
1.0. March 2021
1 / 11
General information
Product Owner of the declaration:
Leca® Uno, Leca Portugal Leca International
Contact person: Tone Storbråten
Phone: +47 41 43 71 00
e-mail: info@leca.no
Program operator: Manufacturer:
Post Box 5250 Majorstuen, 0303 Oslo, Norway Leca International
The Norwegian EPD Foundation Årnesvegen 1
Phone: +47 23 08 80 00 2009 Nordby, Norway
web: post@epd-norge.no
Declaration number: Place of production:
Leca Portugal
Avelar Estrada Nacional N.º 110, s/n Tojeira
3240-356 Avelar Portugal, Portugal
This declaration is based on Product Category Rules: Management system:
CEN Standard EN 15804:2012+A2:2019 serves as core PCR ISO 14001ISO 9001
NPCR Part A: Construction products and services. Ver. 1.0. March
2021
Statement of liability: Organisation no:
The owner of the declaration shall be liable for the underlying 918 799 141
information and evidence. EPD Norway shall not be liable with respect
to manufacturer information, life cycle assessment data and
evidences.​
Declared unit: Issue date:
1 m3 Leca® Uno, Leca Portugal
Declared unit with option: Valid to:
A1,A2,A3,A4,C1,C2,C3,C4,D
Year of study:
2021
Functional unit: Comparability:
EPD of construction products may not be comparable if they not
comply with EN 15804 and seen in a building context.
General information on verification of EPD from EPD tools: Development and verification of EPD:
Independent verification of data, other environmental information The declaration is created using EPD tool lca.tools ver EPD2022.03,
and the declaration according to ISO 14025:2010, § 8.1.3 and § 8.1.4. developed by LCA.no. The EPD tool is integrated in the company's
Individualthird party verification of each EPD is not required when the management system, and has been approved by EPD Norway.
EPD tool is i) integrated into the company's environmental
management system, ii) the procedures for use of the EPD tool are Developer of EPD: Ana Raquel Fernandes
approved by EPDNorway, and iii)the proccess is reviewed annualy. See
Reviewer of company-specific input data and EPD:​ Tone Storbråten
Appendix G of EPD-Norway's General Programme Instructions for
further information on EPD tools.
Verification of EPD tool: Approved:
Independent third party verification of the EPD tool, background data
and test-EPD in accordance with EPDNorway's procedures and
guidelines for verification and approval of EPD tools. Approval
number: NEPDT08
Third party verifier:
Anne Rønning, Norsus AS Håkon Hauan, CEO EPD-Norge
(no signature required)
2 / 11
Product
Product description:
Hydraulic binder based mortar for use on floors in construction. This product is produced with a mix of lightweight expanded clay aggregate with a
particle size between 1 mm and 5 mm, with hydraulic binder and additives. It can be used on floors in construction, indoor or outdoor. The
product is sold in 25 L bags , with the approximately weight of 17 Kg. In total, each pallet has 40 bags.
Product specification
Lightweight mortar for filling and levelling indoor and outdoor floors, applied in a single layer. It allows thermal and acoustic improvement of the
floor. Suitable for application in new construction and rehabilitation projects, in thicknesses from 5 cm.
Materials Value Unit
Leca® expanded clay 84 % (v/v)
Recycled binder 16 % (v/v)
Wooden pallet 1 unit per DU
Plastic packaging 6 Kg per DU
Technical data:
The relevant technical properties for Leca® Uno (after applied) are provided below:
- Compressive strength 28 days: more than 5 N/mm² (5 MPa)
- Flexural strength 28 days: more than 2 N/mm² (2 MPa)
- Reaction to fire: non-combustible (Class A1)
- Density (final product applied - dry basis): 826 ± 2 kg/m³
- Thermal conductivity (according to EN 1745-2002), dry = 0.30 - 0.32 W/m.K
Market:
Portugal and Spain.
Reference service life, product
Not relevant.
Reference service life, building or construction works
Not relevant.
LCA: Calculation rules
Declared unit:
1 m3 Leca® Uno, Leca Portugal
Cut-off criteria:
All major raw materials and all the essential energy is included. The production processes for raw materials and energy flows with very small
amounts (less than 1%) are not included. These cut-off criteria do not​ apply for hazardous materials and substances.
Allocation:
The allocation is made in accordance with the provisions of EN 15804. Incoming energy and water and waste production in-house is allocated
equally among all products through mass allocation. Effects of primary production of recycled materials is allocated to the main product in which
the material was used. The recycling process and transportation of the material is allocated to this analysis.
Data quality:
Specific data for the product composition are provided by the manufacturer. The data represent the production of the declared product and were
collected for EPD development in the year of study. Background data is based on EPDs according to EN 15804 and different LCA databases. The
data quality of the raw materials in A1 is presented in the table below.
Materials Source Data quality Year
Binder ecoinvent 3.6 Database 2019
Packaging ecoinvent 3.6 Database 2019
Packaging Modified ecoinvent 3.6 Database 2019
Dolomite ecoinvent 3.6 Database 2019
Clay LCA.no Database 2021
Waste products LCA.no Database 2021
3 / 11
System boundaries (X=included, MND=module not declared, MNR=module not relevant)
Construction Beyond the system
Product stage Use stage End of life stage
installation stage boundaries
A1 A2 A3 A4 A5 B1 B2 B3 B4 B5 B6 B7 C1 C2 C3 C4 D
X X X X MND MND MND MND MND MND MND MND X X X X X
System boundary:
Additional technical information:
waR slairetam tropsnarT gnirutcafunaM tropsnarT ylbmessA e​sU ecnanetniaM riapeR tnemecalpeR tnemhsibrufeR lanoitarepO ygrene esu lanoitarepO esu retaw -eD noitcurtsnoc noitilomed tropsnarT etsaW gnissecorp lasopsiD -yrevoceR-esueR laitnetop-gnilcyceR
4 / 11
LCA: Scenarios and additional technical information
The following information describe the scenarios in the different modules of the EPD.
Capacity utilisation Value
Transport from production place to user (A4) Distance (km) Fuel/Energy Consumption Unit
(incl. return) % (Liter/tonne)
Truck, 16-32 tonnes, EURO 5 (km) 36,7 % 400 0,044 l/tkm 17,60
De-construction demolition (C1) Unit Value
Demolition of building per kg of LWA block (kg) kg/DU 826,00
Capacity utilisation Value
Transport to waste processing (C2) Distance (km) Fuel/Energy Consumption Unit
(incl. return) % (Liter/tonne)
Truck, 16-32 tonnes, EURO 5 (km) 38,8 % 50 0,045 l/tkm 2,25
Waste processing (C3) Unit Value
Waste treatment per kg of LWA block after
kg 619,50
demolition (kg)
Disposal (C4) Unit Value
Disposal, landfilling of waste LWA (kg) kg 206,50
Benefits and loads beyond the system
Unit Value
boundaries (D)
Substitution of primary aggregates (kg) kg 619,50
5 / 11
LCA: Results
The LCA results are presented below for the declared unit defined on page 2 of the EPD document.
Environmental impact
Indicator Unit A1 A2 A3 A4 C1 C2 C3 C4 D
GWP-total kg CO2 -eq 1,85E+02 5,64E+00 1,22E+01 4,57E+01 3,30E+00 5,71E+00 4,46E-01 1,70E+00 -1,45E+00
GWP-fossil kg CO2 -eq 2,15E+02 5,63E+00 1,20E+01 4,57E+01 3,30E+00 5,71E+00 4,40E-01 1,69E+00 -1,42E+00
GWP-biogenic kg CO2 -eq -3,01E+01 2,30E-03 4,64E-02 1,86E-02 6,20E-04 0,00E+00 3,80E-03 1,98E-03 -2,83E-02
GWP-luluc kg CO2 -eq 2,04E-01 1,97E-03 1,65E-01 1,60E-02 2,61E-04 2,00E-03 6,09E-04 4,16E-04 -9,59E-04
ODP kg CFC11 -eq 1,46E-05 1,28E-06 6,19E-07 1,04E-05 7,14E-07 1,27E-06 8,67E-08 6,41E-07 -2,58E-07
AP mol H+ -eq 1,21E+00 2,30E-02 1,01E-01 1,87E-01 3,46E-02 2,33E-02 3,56E-03 1,51E-02 -1,28E-02
EP-FreshWater kg P -eq 5,86E-03 4,43E-05 5,91E-04 3,59E-04 1,20E-05 4,49E-05 2,78E-05 1,92E-05 -3,77E-05
EP-Marine kg N -eq 3,06E-01 6,83E-03 1,31E-02 5,54E-02 1,53E-02 6,92E-03 1,04E-03 5,60E-03 -4,43E-03
EP-Terrestial mol N -eq 3,52E+00 7,55E-02 1,49E-01 6,12E-01 1,65E-01 7,64E-02 1,20E-02 6,18E-02 -5,20E-02
POCP kg NMVOC -eq 1,01E+00 2,31E-02 4,06E-02 1,87E-01 4,60E-02 2,34E-02 3,22E-03 1,77E-02 -1,37E-02
ADP-minerals&metals1 kg Sb -eq 6,75E-04 1,53E-04 7,73E-05 1,24E-03 5,07E-06 1,54E-04 5,58E-06 1,53E-05 -1,26E-04
ADP-fossil1 MJ 2,26E+03 8,50E+01 1,50E+02 6,89E+02 4,55E+01 8,61E+01 1,37E+01 4,66E+01 -2,40E+01
WDP1 m3 4,64E+03 8,11E+01 -2,54E+03 6,57E+02 9,66E+00 8,21E+01 1,51E+03 2,88E+02 -1,13E+03
GWP total Global Warming Potential total; GWP fossil Global Warming Potential fossil fuels ; GWP biogenic Global Warming Potential biogenic; GWP luluc Global W
Potential land use change; ODP Ozone Depletion; AP Acidification; EP freshwater Eutrophication aquatic freshwater; EP marine Eutrophication aquatic marine; EP
terrestrial Eutrophication terrestrial ;POCP Photochemical zone formation; ADPE Abiotic Depletion Potential minerals and metals; ADPf Abiotic Depletion Potential fossil
fuels;
"Reading example: 9,0 E-03 = 9,0*10-3 = 0,009"
*INA Indicator Not Assessed
1. The results of this environmental impact indicator shall be used with care as the uncertainties on these results are high or as there is limited experienced with the
indicator
Remarks to environmental impacts
Due to polluter-pay-principle, the emissions from waste are not included.
Biogenic carbon from biofuels are balanced to zero since they have their input and output in the same module.
6 / 11
Additional environmental impact indicators
Indicator Unit A1 A2 A3 A4 C1 C2 C3 C4 D
PM Disease incidence 2,35E-05 4,06E-07 2,43E-07 3,29E-06 4,18E-06 3,77E-07 5,70E-08 3,22E-07 -2,72E-07
IRP2 kgBq U235 -eq 6,33E+00 3,71E-01 3,20E-01 3,01E+00 1,98E-01 3,77E-01 2,29E-01 2,13E-01 -2,20E-01
ETP-fw1 CTUe 4,87E+03 6,26E+01 2,16E+02 5,07E+02 2,49E+01 6,34E+01 9,68E+00 2,54E+01 -2,47E+01
HTP-c1 CTUh 9,33E-08 0,00E+00 4,55E-09 0,00E+00 8,26E-10 0,00E+00 6,20E-10 1,03E-09 -1,24E-09
HTP-nc1 CTUh 1,49E-06 6,76E-08 1,66E-07 5,48E-07 2,31E-08 6,85E-08 8,67E-09 1,84E-08 -3,04E-08
SQP1 dimensionless 5,65E+03 5,86E+01 5,16E+01 4,75E+02 5,53E+00 5,94E+01 7,73E+00 1,79E+02 5,45E+01
PM Particulate Matter emissions; IRP Ionizing radiation – human health; ETP-fw Eco toxicity – freshwater; HTP-c Human toxicity – cancer effects; HTP-nc Human
toxicity – non cancer effects; SQP Soil Quality (dimensionless)
"Reading example: 9,0 E-03 = 9,0*10-3 = 0,009"
*INA Indicator Not Assessed
1. The results of this environmental impact indicator shall be used with care as the uncertainties on these results are high or as there is limited experienced with the
indicator
2. This impact category deals mainly with the eventual impact of low dose ionizing radiation on human health of the nuclear fuel cycle. It does not consider effects due
to possible nuclear accidents, occupational exposure nor due to radioactive waste disposal in underground facilities. Potential ionizing radiation from the soil, from
radon and from some construction materials is also not measured by this indicator.
7 / 11
Resource use
Indicator Unit A1 A2 A3 A4 C1 C2 C3 C4 D
PERE MJ 7,86E+02 1,20E+00 8,30E+01 9,72E+00 2,48E-01 1,22E+00 7,03E+00 1,67E+00 -5,62E+00
PERM MJ 2,78E+02 0,00E+00 0,00E+00 0,00E+00 0,00E+00 0,00E+00 0,00E+00 0,00E+00 0,00E+00
PERT MJ 1,06E+03 1,20E+00 8,30E+01 9,72E+00 2,48E-01 1,22E+00 7,03E+00 1,67E+00 -5,62E+00
PENRE MJ 2,00E+03 8,50E+01 1,50E+02 6,89E+02 4,55E+01 8,67E+01 1,37E+01 4,66E+01 -2,53E+01
PENRM MJ 2,58E+02 0,00E+00 0,00E+00 0,00E+00 0,00E+00 0,00E+00 0,00E+00 0,00E+00 0,00E+00
PENRT MJ 2,26E+03 8,50E+01 1,50E+02 6,89E+02 4,55E+01 8,67E+01 1,37E+01 4,66E+01 -2,53E+01
SM kg 1,22E+00 0,00E+00 1,46E-03 0,00E+00 2,23E-02 3,46E-02 1,17E-02 0,00E+00 -4,85E-02
RSF MJ 4,17E+00 4,29E-02 6,20E-02 3,48E-01 6,05E-03 4,35E-02 1,42E-01 3,46E-02 -1,15E-01
NRSF MJ 1,53E+01 1,53E-01 8,79E-03 1,24E+00 -9,09E-02 1,55E-01 -8,83E-03 7,48E-02 -1,18E-01
FW m3 1,07E+00 8,95E-03 1,32E-01 7,25E-02 2,34E-03 9,08E-03 2,34E-02 5,74E-02 -8,81E-01
PERE Use of renewable primary energy excluding renewable primary energy resources used as raw materials; PERM Use of renewable primary energy resources used as
raw materials; PERT Total use of renewable primary energy resources; PENRE Use of non renewable primary energy excluding non-renewable primary energy resources
used as raw materials; PENRM Use of non renewable primary energy resources used as raw materials; PENRT Total use of non renewable primary energy resources; SM
Use of secondary materials; RSF Use of renewable secondary fuels; NRSF Use of non renewable secondary fuels; FW Use of net fresh water
"Reading example: 9,0 E-03 = 9,0*10-3 = 0,009"
*INA Indicator Not Assessed
8 / 11
End of life - Waste
Indicator Unit A1 A2 A3 A4 C1 C2 C3 C4 D
HWD kg 3,80E-01 4,33E-03 5,11E-02 3,51E-02 1,34E-03 4,38E-03 1,36E-03 0,00E+00 -5,78E-03
NHWD kg 8,16E+00 4,06E+00 7,37E-01 3,29E+01 5,39E-02 4,11E+00 4,31E-02 2,07E+02 -1,75E-01
RWD kg 7,87E-03 5,79E-04 2,85E-04 4,70E-03 3,16E-04 5,86E-04 1,44E-04 0,00E+00 -1,90E-04
HWD = Hazardous waste disposed; NHWD = Non-hazardous waste disposed; RWD = Radioactive waste disposed;
"Reading example: 9,0 E-03 = 9,0*10-3 = 0,009"
*INA Indicator Not Assessed
End of life - Output flow
Indicator Unit A1 A2 A3 A4 C1 C2 C3 C4 D
CRU kg 0,00E+00 0,00E+00 0,00E+00 0,00E+00 0,00E+00 0,00E+00 0,00E+00 0,00E+00 0,00E+00
MFR kg 4,76E-01 0,00E+00 3,25E-01 0,00E+00 2,19E-02 4,83E-04 6,20E+02 0,00E+00 -1,14E-03
MER kg 3,29E-02 0,00E+00 4,19E-06 0,00E+00 6,80E-05 2,88E-02 1,43E-03 0,00E+00 -4,25E-02
EEE MJ 1,02E-01 0,00E+00 8,40E-02 0,00E+00 2,33E-04 3,33E-03 2,45E-03 0,00E+00 -1,03E-02
EET MJ 1,55E+00 0,00E+00 1,27E+00 0,00E+00 3,53E-03 5,03E-02 3,70E-02 0,00E+00 -1,55E-01
CRU = Components for re-use; MFR = Materials for recycling; MER = Materials for energy recovery; EEE = Exported electrical energy; EET = Exported energy ​ Thermal
"Reading example: 9,0 E-03 = 9,0*10-3 = 0,009"
*INA Indicator Not Assessed
Biogenic Carbon Content
Indicator Unit At the factory gate
Biogenic carbon content in product kg C 0,00E+00
Biogenic carbon content in accompanying packaging kg C 8,27E+00
Note: 1 kg biogenic carbon is equivalent to 44/12 kg CO2
9 / 11
Additional Norwegian requirements
Greenhouse gas emissions from the use of electricity in the manufacturing phase
National production mix from import, low voltage (production of transmission lines, in addition to direct emissions and losses in grid) of applied
electricity for the manufacturing process (A3).
Electricity mix Data source Amount Unit
Electricity, Portugal (kWh) ecoinvent 3.6 405,87 g CO2-eq/kWh
Dangerous substances
The product contains no substances given by the REACH Candidate list or the Norwegian priority list.
Indoor environment
Additional Environmental Information
Environmental impact indicators EN 15804+A1 and NPCR Part A v2.0
Indicator Unit A1 A2 A3 A4 C1 C2 C3 C4 D
GWP kg CO2 -eq 2,14E+02 5,58E+00 1,26E+01 4,52E+01 3,26E+00 5,69E+00 4,34E-01 1,66E+00 -1,52E+00
ODP kg CFC11 -eq 1,23E-05 1,01E-06 5,77E-07 8,22E-06 5,67E-07 1,03E-06 1,07E-07 5,16E-07 -2,35E-07
POCP kg C2H4 -eq 1,66E-01 7,45E-04 3,21E-03 6,04E-03 5,03E-04 7,55E-04 9,64E-05 3,90E-04 -3,16E-04
AP kg SO2 -eq 9,26E-01 1,11E-02 8,52E-02 8,97E-02 4,83E-03 1,12E-02 1,63E-03 4,61E-03 -3,71E-03
EP kg PO43- -eq 1,30E-01 1,18E-03 6,35E-03 9,57E-03 5,37E-04 1,20E-03 2,16E-04 5,44E-04 -4,35E-04
ADPM kg Sb -eq 6,75E-04 1,53E-04 7,73E-05 1,24E-03 5,07E-06 1,55E-04 5,58E-06 1,53E-05 -1,26E-04
ADPE MJ 2,11E+03 8,32E+01 1,50E+02 6,75E+02 4,52E+01 8,61E+01 5,25E+00 4,47E+01 -2,40E+01
GWPIOBC kg CO2 -eq 4,92E+01 5,64E+00 1,25E+01 4,57E+01 4,43E+03 5,69E+00 0,00E+00 0,00E+00 -1,52E+00
GWP Global warming potential; ODP Depletion potential of the stratospheric ozone layer; POCP Formation potential of tropospheric photochemical oxidants; AP
Acidification potential of land and water; EP Eutrophication potential; ADPM Abiotic depletion potential for non fossil resources; ADPE Abiotic depletion​ potential for
fossil resources; GWP-IOBC/GHG Global warming potential calculated according to the principle of instantanious oxidation (except emissions and uptake of biogenic
carbon)
10 / 11
Bibliography
ISO 14025:2010 Environmental labels and declarations - Type III environmental declarations - Principles and procedures.
ISO 14044:2006 Environmental management - Life cycle assessment - Requirements and guidelines.
EN 15804:2012+A2:2019 Environmental product declaration - Core rules for the product category of construction products.
ISO 21930:2017 Sustainability in buildings and civil engineering works - Core rules for environmental product declarations of construction
products.
ecoinvent v3, Allocation, cut-off by classification, Swiss Centre of Life Cycle Inventories.
Iversen et al., (2021) eEPD v2021.09 Background information for EPD generator tool system verification, LCA.no Report number: 07.21
Iversen et al., (2018) EPD generator for Leca - Background information for customer application, LCA.no report number 06.18
NPCR Part A: Construction products and services. Ver. 2.0. April 2021, EPD-Norge.
Program operator and publisher Phone: +47 23 08 80 00
The Norwegian EPD Foundation e-mail: post@epd-norge.no
Post Box 5250 Majorstuen, 0303 Oslo, Norway web: www.epd-norge.no
Owner of the declaration: Phone: +47 41 43 71 00
Leca International e-mail: info@leca.no
Årnesvegen 1, 2009 Nordby web: www.leca.no
Author of the Life Cycle Assessment Phone: +47 916 50 916
LCA.no AS e-mail: post@lca.no
Dokka 6B, 1671 web: www.lca.no
Developer of EPD generator Phone: +47 916 50 916
LCA.no AS e-mail: post@lca.no
Dokka 6B,1671 Kråkerøy web: www.lca.no
ECO Platform web: www.eco-platform.org
ECO Portal web: ECO Portal
11 / 11
