ver1 2015
ENVIRONMENTAL PRODUCT DECLARATION
in accordance with ISO 14025, ISO 21930 and EN 15804
Owner of the declaration: Lindab P rofil A B
Program operator: T he Norwegian EP D Foundation
Publisher: T he Norwegian EP D Foundation
Declaration number: NEPD-2269-1037-EN
Registration number: NEPD-2269-1037-EN
ECO Platform reference number: -
Issue date: 29.06.2020
Valid to: 29.06.2025
Lindab ConstruLine
Lindab Profil AB
www.epd-norge.no
NEPD-2269-1037-EN Lindab ConstruLine 1 / 8
General information
Product: Owner of the declaration:
Lindab ConstruLine Lindab Profil AB
Contact person: Lina Hedvall
Phone: +46 (431) 85132
e-mail: lina.hedvall@lindab.com
Program operator: Manufacturer:
T he Norwegian EP D Foundation Lindab Profil AB
P b. 5250 M ajorstuen, 0303 O slo
P hone: +47 23 08 80 00
e-mail: post@epd-norge.no
Declaration number: Place of production:
Lindab Profil Förslöv
NEPD-2269-1037-EN
ECO Platform reference number: Management system:
SE006902-1 ISO 9001:2015 SE006898-1 ISO 14001:2015
This declaration is based on Product Category Rules: Organisation no:
556247-2273
CEN Standard EN 15804:2012+A1:2013 serves as core PCR
NPCR 013:2019 Part B for Steel and aluminium construction
products
Statement of liability: Issue date:
The owner of the declaration shall be liable for the underlying 29.06.2020
information and evidence. EPD Norway shall not be liable with
respect to manufacturer information, life cycle assessment data Valid to:
and evidences.
29.06.2025
Declared unit: Year of study:
1 kg Lindab ConstruLine 2020
Declared unit with option: Comparability:
EPD of construction products may not be comparable if they not
A1,A2,A3,A4,A5,C2,C3,C4,D
comply with EN 15804 and seen in a building context.
Functional unit: Author of the Life Cycle Assessment:
The declaration is developed using eEPD v4.0 from LCA.no
Approval:
Company specific data are:
Collected/registered by: Carina Petersson
Internal verification by: Lina Hedvall
Verification: Approved:
Independent verification of data, other environmental information
and the declaration according to ISO14025:2010, § 8.1.3 and §
8.1.4
External
Third party verifier:
Sign Sign
Fredrik Moltu Johnsen
(Independent verifier approved by EPD Norway)
NEPD-2269-1037-EN Lindab ConstruLine 2 / 8
Product
Product description: Technical data:
Lindabs beams, battens, studs and runners are manufactured from Declaration of Performance C-profiles:
hot dip galvanized steel with different surface treatment in order to https://itsolution.lindab.com/lindabwebproductsdoc/pdf/documentation/building_components/uk/DoP/C_profiles.pdf
obtain requested corrosion protection properties.The products Declaration of Performance exterior and interior studs and runners:
connected to these systems are primarily used as a base or https://itsolution.lindab.com/lindabwebproductsdoc/pdf/documentation/building_components/uk/dop/Declaration_of_Performance_Partition_Wall_Profiles.pdf
framework in the construction of interior walls, exterior walls and Declaration of Performance U-profiles:
ceilings. This EPD covers the zinc coated products. https://itsolution.lindab.com/lindabwebproductsdoc/pdf/documentation/building_components/uk/dop/Declaration_of_Performance_U_Profiles.pdf
Declaration of Performance Z-profiles:
Product specification
https://itsolution.lindab.com/lindabwebproductsdoc/pdf/documentation/building_components/uk/dop/Declaration_of_Performance_Z_Profiles.pdf
The steel grade used for this product is S350GD Z275 and FA Z100.
The nominal thickness varies from 0,52 to 3,0mm depending on Market:
product and area of use. The beams, battens, studs and runners are maily sold in
Scandinavia.
Materials %
Packaging 2,79 Reference service life, product
Steel 97,21
60 years
Reference service life, building
60 years
LCA: Calculation rules
Declared unit: Allocation:
The allocation is made in accordance with the provisions of EN
1 kg Lindab ConstruLine
15804. Incoming energy and water and waste production in-house is
Cut-off criteria: allocated equally among all products through mass allocation.
Effects of primary production of recycled materials is allocated to the
All major raw materials and all the essential energy is included. The
main product in which the material was used. The recycling process
production processes for raw materials and energy flows with very
and transportation of the material is allocated to this analysis.
small amounts (less than 1%) are not included. These cut-off criteria
do not apply for hazardous materials and substances.
Data quality:
Specific data for the product composition are provided by the manufacturer. They represent the production of the declared product and were
collected for EPD development in the year of study. Background data is based on registered EPDs according to EN 15804, Ostfold Research
databases, ecoinvent and other LCA databases. The data quality of the raw materials in A1 is presented in the table below.
For A1-A4 the data is actual data or suggestions from the c-CPR. For the other modules conservative assumptions have been made.
Materials Source Data quality Year
Steel EPD-ARM-20170139-IBD1-EN EPD 2017
Packaging ecoinvent 3.5 Database 2018
NEPD-2269-1037-EN Lindab ConstruLine 3 / 8
System boundary:
Module A1-A5, C2-C4 and D is included in the analysis. That means everything except the usage stage and assembly. That is excluded
since the product has very limited effect on the environment during this phase of its lifetime. C1 is excluded since the work method varies
greatly between different projects and the energy consumption is negotiable from a life cycle perspective. For the same reason energy
consumption during construction has been excluded.
Additional technical information:
NEPD-2269-1037-EN Lindab ConstruLine 4 / 8
LCA: Scenarios and additional technical information
The following information describe the scenarios in the different modules of the EPD.
The after life scenario assumes 100% recycling of steel. The same energy consumption has been assumed for assembly and deconstruction.
During assembly no scrap has been assumed since the product is custom made in the right dimensions for each construction.
Transport from production place to user (A4)
Capacity
Fuel/Energy
Type utilisation (incl. Type of vehicle Distance km Unit Value (l/t)
consumption
return) %
Truck, lorry 16-32
Truck 38,8 % 300 0,044606 l/tkm 13,38
tonnes, EURO 5
Railway l/tkm
Boat l/tkm
Other Transportation l/tkm
Assembly (A5) End of Life (C1, C3, C4)
. Unit Value . Unit Value
Auxiliary kg Hazardous waste disposed kg
Water consumption m3 Collected as mixed construction waste kg
Electricity consumption kWh Reuse kg
Other energy carriers MJ Recycling kg 1,0000
Material loss kg Energy recovery kg
Output materials from waste treatment kg 0,0300 To landfill kg
Dust in the air kg
VOC emissions kg
Transport to waste processing (C2)
Capacity
Fuel/Energy
Type utilisation (incl. Type of vehicle Distance km Unit Value (l/t)
consumption
return) %
Truck, lorry 16-32
Truck 38,8 % 100 0,044606 l/tkm 4,46
tonnes, EURO 5
Railway l/tkm
Boat l/tkm
Other Transportation l/tkm
¨
Benefits and loads beyond the system boundaries (D)
. Unit Value
Substitution of primary construction steel, with net scrap steel (kg) kg/DU 0,92
NEPD-2269-1037-EN Lindab ConstruLine 5 / 8
LCA: Results
System boundaries (X=included, MND=module not declared, MNR=module not relevant)
Construction Beyond the
Product stage installation User stage End of life stage . system
stage bondaries
A1 A2 A3 A4 A5 B1 B2 B3 B4 B5 B6 B7 C1 C2 C3 C4 . D
X X X X X MNR MNR MNR MNR MNR MNR MNR MNR X X X . X
Environmental impact
Parameter Unit A1-A3 A4 A5 C2 C3 C4 D
GWP kg CO 2 -eq 2,79E+00 4,88E-02 9,80E-04 1,63E-02 2,00E-04 0 -1,54E+00
ODP kg CFC11 -eq 1,15E-08 9,00E-09 1,12E-10 3,00E-09 2,20E-11 0 -6,34E-08
POCP kg C 2H 4-eq 8,02E-04 7,95E-06 2,00E-07 2,65E-06 5,48E-08 0 -1,07E-03
AP kg SO 2 -eq 5,39E-03 1,56E-04 5,13E-06 5,19E-05 1,25E-06 0 -6,87E-03
EP kg PO 3- -eq 5,69E-04 2,58E-05 1,32E-06 8,61E-06 1,92E-07 0 -2,29E-03
4
ADPM kg Sb -eq 1,45E-04 1,49E-07 1,72E-09 4,96E-08 1,50E-11 0 -2,97E-05
ADPE MJ 2,54E+01 7,35E-01 1,17E-02 2,45E-01 1,86E-03 0 -1,45E+01
GWP Global warming potential; ODP Depletion potential of the stratospheric ozone layer; POCP Formation potential of tropospheric photochemical
oxidants; AP Acidification potential of land and water; EP Eutrophication potential; ADPM Abiotic depletion potential for non fossil resources; ADPE
Abiotic depletion potential for fossil resources
Reading example: 9,0 E-03 = 9,0*10-3 = 0,009
*INA Indicator Not Assessed
waR slairetam tropsnarT gnirutcafunaM tropsnarT ylbmessA esU ecnanetniaM riapeR tnemecalpeR tnemhsibrufeR lanoitarepO ygrene esu lanoitarepO esu
retaw
-eD noitcurtsnoc noitilomed tropsnarT etsaW gnissecorp lasopsiD -yrevoceR-esueR -gnilcyceR laitnetop
NEPD-2269-1037-EN Lindab ConstruLine 6 / 8
Resource use
Parameter Unit A1-A3 A4 A5 C2 C3 C4 D
RPEE MJ 2,43E+00 1,07E-02 2,69E-01 3,57E-03 1,55E-02 0 -1,30E+00
RPEM MJ 4,23E-01 0,00E+00 0,00E+00 0,00E+00 0,00E+00 0 0,00E+00
TPE MJ 2,85E+00 1,07E-02 2,69E-01 3,57E-03 1,55E-02 0 -1,30E+00
NRPE MJ 2,75E+01 7,53E-01 1,28E-02 2,51E-01 2,50E-03 0 -1,37E+01
NRPM MJ 0,00E+00 0,00E+00 0,00E+00 0,00E+00 0,00E+00 0 0,00E+00
TRPE MJ 2,75E+01 7,53E-01 1,28E-02 2,51E-01 2,50E-03 0 -1,37E+01
SM kg 8,38E-02 0,00E+00 0,00E+00 0,00E+00 0,00E+00 0 0,00E+00
RSF MJ 5,68E-04 0,00E+00 0,00E+00 0,00E+00 0,00E+00 0 0,00E+00
NRSF MJ 0,00E+00 0,00E+00 0,00E+00 0,00E+00 0,00E+00 0 0,00E+00
W m3 9,00E-03 1,41E-04 7,17E-06 4,70E-05 1,03E-06 0 -9,40E-03
RPEE Renewable primary energy resources used as energy carrier; RPEM Renewable primary energy resources used as raw materials; TPE Total use
of renewable primary energy resources; NRPE Non renewable primary energy resources used as energy carrier; NRPM Non renewable primary energy
resources used as materials; TRPE Total use of non renewable primary energy resources; SM Use of secondary materials; RSF Use of renewable
secondary fuels; NRSF Use of non renewable secondary fuels; W Use of net fresh water
Reading example: 9,0 E-03 = 9,0*10-3 = 0,009
*INA Indicator Not Assessed
End of life - Waste
Parameter Unit A1-A3 A4 A5 C2 C3 C4 D
HW kg 1,50E-03 4,40E-07 1,51E-08 1,47E-07 6,18E-09 0 -1,33E-04
NHW kg 8,57E-02 3,96E-02 9,15E-04 1,32E-02 1,90E-04 0 -2,64E+00
RW kg INA* INA* INA* INA* INA* 0 INA*
HW Hazardous waste disposed; NHW Non hazardous waste disposed; RW Radioactive waste disposed
Reading example: 9,0 E-03 = 9,0*10-3 = 0,009
*INA Indicator Not Assessed
End of life - Output flow
Parameter Unit A1-A3 A4 A5 C2 C3 C4 D
CR kg 0,00E+00 0,00E+00 0,00E+00 0,00E+00 0,00E+00 0 0,00E+00
MR kg 4,70E-02 0,00E+00 1,08E-02 0,00E+00 0,00E+00 0 0,00E+00
MER kg 0,00E+00 0,00E+00 0,00E+00 0,00E+00 0,00E+00 0 0,00E+00
EEE MJ INA* INA* INA* INA* INA* 0 INA*
ETE MJ INA* INA* INA* INA* INA* 0 INA*
CR Components for reuse; MR Materials for recycling; MER Materials for energy recovery; EEE Exported electric energy; ETE Exported thermal
energy
Reading example: 9,0 E-03 = 9,0*10-3 = 0,009
*INA Indicator Not Assessed
NEPD-2269-1037-EN Lindab ConstruLine 7 / 8
Additional Norwegian requirements
Greenhouse gas emissions from the use of electricity in the manufacturing phase
National production mix from import, low voltage (production of transmission lines, in addition to direct emissions and losses in grid) of
applied electricity for the manufacturing process (A3).
Electricity mix Data source Amount Unit
El-mix, Sweden (kWh) ecoinvent 3.4 Alloc Rec 42,67 g CO2-ekv/kWh
Dangerous substances
The product contains no substances given by the REACH Candidate list or the Norwegian priority list.
Indoor environment
The product has no effect on the Indoor Environment.
Bibliography
ISO 14025:2010 Environmental labels and declarations - Type III environmental declarations - Principles and procedures.
ISO 14044:2006 Environmental management - Life cycle assessment - Requirements and guidelines.
EN 15804:2012+A1:2013 Environmental product declaration - Core rules for the product category of construction products.
ISO 21930:2017 Sustainability in buildings and civil engineering works - Core rules for environmental product declarations of construction
products.
ecoinvent v3, Allocation, cut-off by classification, Swiss Centre of Life Cycle Inventories.
Iversen et al., (2018) eEPD v3.0 - Background information for EPD generator system. LCA.no report number 04.18.
Vold et al., (2019) EPD generator for Norsk Stålforbund - Background information and LCA data, LCA.no report number 09.19.
NPCR Part A: Construction products and services. Ver. 1.0. April 2017, EPD-Norge.
NPCR 013 Part B for steel and aluminium construction products. Ver. 3.0 April 2019, EPD-Norge.
Bucht & Korhonen, Communication and knowledge for decreased energy consumption during the production phase, 2018, Jönköping
University
Program operator and publisher Phone: +47 23 08 80 00
The Norwegian EPD Foundation
Post Box 5250 Majorstuen, 0303 Oslo e-mail: post@epd-norge.no
0303 Oslo Norway web: www.epd-norge.no
Owner of the declaration Phone: +46 (431) 85132
Lindab Profil AB Fax:
Vistorpsvägen 56 e-mail: lina.hedvall@lindab.com
269 71 Förslöv web: www.lindab.se
Author of the Life Cycle Assessment Phone: +47 916 50 916
LCA.no AS Fax:
Dokka 1C e-mail: post@lca.no
1671 Kråkerøy web: www.lca.no
Developer of EPD generator Phone: +47 916 50 916
LCA.no AS
Dokka 1C e-mail: post@lca.no
1671 Kråkerøy web: www.lca.no
NEPD-2269-1037-EN Lindab ConstruLine 8 / 8
