ENVIRONMENTAL PRODUCT DECLARATION
as per ISO 14025 and EN 15804+A2
Owner of the Declaration Grundfos Holding A/S
Publisher Institut Bauen und Umwelt e.V. (IBU)
Programme holder Institut Bauen und Umwelt e.V. (IBU)
Declaration number EPD-GRU-20230074-CBC1-EN
Issue date 22/11/2023
Valid to 21/11/2028
MAGNA3 100-40/60 (Cast Iron)
Grundfos Holding A/S
www.ibu-epd.com | https://epd-online.com
General Information
Grundfos Holding A/S MAGNA3 100-40/60 (Cast Iron)
Programme holder Owner of the declaration
IBU – Institut Bauen und Umwelt e.V. Grundfos Holding A/S
Hegelplatz 1 Poul Due Jensens Vej 7
10117 Berlin 8850 Bjerringbro
Germany Denmark
Declaration number Declared product / declared unit
EPD-GRU-20230074-CBC1-EN 1 PCS. of MAGNA3 100-40/60 (Cast Iron)
This declaration is based on the product category rules: Scope:
Pumps for liquids and liquids with solids, 01/08/2021 The declaration applies to 1 piece of MAGNA3 (Cast Iron) pump.
(PCR checked and approved by the SVR)
The product is produced in Wahlstedt, Germany, and the life cycle
assessment is based on data collected at the production site.
Issue date
Production has been modeled using annual production data from 2021.
22/11/2023
The declaration covers two different types of the MAGNA3 100- product
(40/60).
Valid to
21/11/2028 The owner of the declaration shall be liable for the underlying information
and evidence; the IBU shall not be liable with respect to manufacturer
information, life cycle assessment data and evidences.
The EPD was created according to the specifications of EN 15804+A2. In
the following, the standard will be simplified as EN 15804.
Verification
The standard EN 15804 serves as the core PCR
Independent verification of the declaration and data according to ISO
14025:2011
Dipl.-Ing. Hans Peters internally X externally
(Chairman of Institut Bauen und Umwelt e.V.)
Florian Pronold Mrs Kim Allbury,
(Managing Director Institut Bauen und Umwelt e.V.) (Independent verifier)
1 Environmental Product Declaration - Grundfos Holding A/S - MAGNA3 100-40/60 (Cast Iron)
Product
Product description/Product definition Ecodesign Directive (2009/125/EC)
The Grundfos MAGNA3 circulator pumps are designed for
circulating liquids in heating systems, air conditioning and Commission Regulation (EC) No: 641/2009 and
cooling systems and domestic hot water systems. However, the
pump range can also be used in ground source heat pump Commission Regulation (EU) 622/2012
systems and solar heating systems.
Standards used:
The MAGNA3 pump is a centrifugal pump powered by an EN 16297-1:2012, EN 16297-2:2012, EN 16297-3:2012.
electrical motor. It has a high-performance neodymium magnet
rotor which increases motor efficiency and an insulation shell to The CE marking takes into account the proof of conformity with
reduce heat loss from the cast iron pump housing with threaded the respective harmonized norms based on the legal provisions
connections. above.
The declaration covers two types of the MAGNA3 pump. They MAGNA3 pumps are not harmonized in accordance with the
are grouped as shown below. The group reference in the CPR.
technical data and scenarios refers also to these.
Application
GROUP 1 - MAGNA3 100-40 For the application and use the respective national provisions
GROUP 2 - MAGNA3 100-60 apply.
These are all the same physical products and 100 % identical The pump is designed for circulating liquids in the following
in terms of design, dimensions and materials as well as supply systems:
chain and manufacturing processes, i.e., all cradle to gate
processes (A1-A3). · heating systems
· domestic hot-water systems
The products are also identical in terms of packaging, · air-conditioning and cooling systems
distribution, reference service life and end-of-life treatment. · ground-source heat-pump systems
· solar-heating systems
The only thing that differentiates the products from each other
is the software which controls how the pump operates in the The pump is suitable for thin, clean, non-aggressive and non-
system in which it is installed, making them fit for different explosive liquids, not containing solid particles or fibres that
applications. Hence, all life cycle modules are identical, except may attack the pump mechanically or chemically. In heating
use stage module B6, which will change, as the applied systems, the water must meet the requirements of accepted
scenarios for electricity consumption changes. For the placing standards on water quality in heating systems. The pumps are
on the market in the European Union/European Free Trade also suitable for domestic hot-water systems.
Association (EU/EFTA) (with the exception of Switzerland) the
following legal provisions apply: Technical Data
The performance data of the product according to the
Machinery Directive (2006/42/EC) harmonized norms, based on the harmonization provisions
above apply.
Standard used: EN 809:1998 + A1:2009. The relevant technical specifications according to the PCR Part
B are given in the table below.
Radio Equipment Directive (2014/53/EU) Characteristics that are the same for all product groups are only
given once. Others are given individually for all two groups.
Standards used: Constructional data
EN 60335-1:2012/AC:2014 + A11:2014, EN 60335-2-51:2003 +
Name Value Unit
A1:2008 + A2:2012, EN 62233:2008.
Frequency 50 Hz
EN 55014-1:2006 + A1:2009 + A2:2011, EN 55014-1:2017, EN Voltage 230 V
61000-6-2:2005, EN 61000-3-2:2014, EN 61000-3-3:2013, Clean
Pumped liquid (e.g. water) -
ETSI EN 301 489-1 V2.2.0, ETSI EN 301 489-17 V3.2.0. ETSI Water
EN 300 328 V2.1.1 Energy Efficiency Index 0,17
Energy Efficiency Index 0,17
Electromagnetic Compatibility (EMC) Directive
Flow range Gr. 1 (max) 50,0 m3/h
(2014/30/EU)
Flow range Gr. 2 (max) 53,0 m3/h
Standards used: Head max. Gr.1 4 m3/h
EN 55014-1:2017, EN 55014-2:2015, Head max. Gr. 2 6 m
Power input Gr. 1 Average (from load profile
EN 61000-3-2:2014/2019, EN 61000-6-2:2008/2019, 0,204 kW
describing use)
Power input Gr. 2 Average (from load profile
EN 61000-3-3:2013 A1:2019 0,257 kW
describing use)
RoHS Directive 2011/65/EU and 2015/863//EU Nominal capacity Gr.1 0,452 kW
Nominal capacity Gr.2 0,65 kW
Standard: EN 50581:2012.
2 Environmental Product Declaration - Grundfos Holding A/S - MAGNA3 100-40/60 (Cast Iron)
Performance data of the product according to the harmonized and ISO 9001.
standards, based on provisions for harmonization.
Reference service life
Base materials/Ancillary materials No use stage scenario which refers to the lifetime of the product
is declared. However, to facilitate building calculations, an
Base materials / Ancillary materials
estimated RSL of 10 years can be used.
Name Value Unit
This is an EU consensus-based estimation, referenced on page
Aluminium 9 % 37 in Appendix 7: Lot 11 – Circulators in Buildings, prepared by
Cast iron 61 % AEA Energy & Environment for the European Commission in
Ceramics 0,2 % the context of the Eco Design Directive:
Copper 3 %
There is no definitive information on the average circulator life
Electronics 0,2 %
available, there is consensus within the industry that it is at
Magnet Nd 1 % least 12 years. However, this is complicated by many factors,
Paper 0,3 % including many being scrapped prematurely when e.g. the
PCB 2 % boiler they are connected to is replaced.
From the estimated stock (140Mpa) and annual sales (14Mpa),
Plastics 0,2 %
the average lifetime of the circulator is taken as 10 years for the
Plastics, foam 1 %
purposes of this study.
Plastics GF 3 % The RSL of the declared product is not directly influencing the
Rubber 0,1 % results in this study, as no declared use stage scenario is
Stainless steel 3 % dependent on the RSL; The use stage sub-module B6 is
Steel 8 % declared per year as required by the PCR Part B.
Cardboard 7 %
Plastic film 0,1 %
TOTAL 100 %
REACH
This product/article/at least one partial article contains
substances listed in the ECHA candidate list (date:
10.06.2022) exceeding 0.1 percentage by mass: no
The Wahlstedt production has been assessed and certified as
meeting the requirements in ISO 14001, ISO 50001, ISO 45001
LCA: Calculation rules
finished product at the gate is rather complex and includes a
Declared Unit large amount of raw materials, components, and semi-finished
The declared unit is 1 piece (pcs.) of MAGNA3 (Cast Iron) parts which come from both external suppliers and other
pump. Grundfos production facilities.
Declared unit The product stage is included in the study, and according to EN
15804 the system boundary with nature is set to include those
Name Value Unit
processes that provide the material and energy inputs into the
Declared unit 1 pce.
system and the following manufacturing, transport up to the
Mass reference 36.6 kg/pce factory gate, as well as the processing of any waste arising
Conversion factor [Mass/Declared Unit] 36.6 from those processes.
Wastes and losses are included in the modules where they
For IBU core EPDs (where clause 3.6 is part of the EPD): for
occur according to the polluter pays principle and the modular
average EPDs, an estimate of the robustness of the LCA
approach of EN 15804.
values must be made, e.g. concerning the variability of the
production process, geographical representativeness and the
The product includes:
influence of background data and preliminary products
compared to the environmental impacts caused by the actual
· A1 Extraction and processing of raw materials;
production.
· A1 Reuse of products or materials from a previous product
system;
System boundary · A1 Processing of secondary materials;
· A1 Generation of electricity, steam and heat from primary
System boundary
energy resources, also including their extraction, refining and
This EPD is Cradle-To-Grave. The system boundaries of the
transport;
EPD follow the modular approach in EN 15804. By decision no.
· A1 Energy recovery and other recovery processes from
20170712-n of the SVR, the modules B3, B4 and B5 are by
secondary fuels;
default declared as "MNR" (module not relevant).
· A2 Transportation up to the factory gate and internal transport;
· A3 Production of ancillary materials or pre products;
The product stage (A1-A3) comprises raw material extraction
· A3 Manufacturing of products and coproducts;
and processing, transport processes, as well as the
· A3 Manufacturing of packaging;
manufacturing process. The final production and assembly of
· A1-A3 processing up to the end-of-waste state or disposal of
the MAGNA3 pump take place at a Grundfos manufacturing
final residues.
site in Germany. However, the full supply chain leading to the
3 Environmental Product Declaration - Grundfos Holding A/S - MAGNA3 100-40/60 (Cast Iron)
impacts and aspects related to the losses during the use stage
For secondary material inputs, the system boundary to the (i.e. production, transport, and waste processing and disposal
previous system (providing the secondary material) is set where of the lost products and materials).
outputs reach the end-of-waste state. The recycling of
secondary material into new raw materials is included in the Generally, the geographical coverage of the datasets used
system boundary of this study. Waste materials from production matches the actual processes taking place. Meaning, that when
processes that are recycled without any modification of the modelling taking place in Grundfos Bjerringbro, the Danish
material's inherent characteristics are modelled as closed loop electricity grid mix is used in the model and thermal energy
within A1-A3. This is done up to the input mass flow that was from natural gas. These are generally of very high quality with
used during production. very good technological, temporal and geographical
Waste for incineration arising in the product stage is accounted representativeness.
for in the module where the waste is produced. The
environmental loads from the incineration process are declared Contributions to operational energy use during the use stage
in the module where it occurs and the electricity and heat which (B6) come from the electricity consumption of the product. The
is produced from the incineration are considered as closed-loop annual electricity consumption is calculated by multiplying the
within A1-A3, as described in PCR Part A, 5.5.1. The input of average power input, which is based on a defined load profile,
biogenic carbon from the production of packaging material is with the annual running hours. For use stage (B6) European
inventoried in A3. As required by PCR Part A, the Average electricity grid mix has been used. These values are
corresponding end-of-life module of the packaging material, A5, declared in the scenarios section.
is also declared and the emissions of biogenic carbon are
inventoried. The End-of-Life stage (C1-C4) includes all activities from
when the product reaches the end of its service life and no
The construction process stage (A4-A5) includes: longer provides any functionality and until all materials and
components are processed for reuse/recycling or disposed of.
A4:
According to EN 15804 and the PCR Part A, the end-of-life
· Transportation from factory gate to distribution center: stage includes:
· Consumption of electricity, thermal energy and water at
distribution center; · C1 deconstruction of the product from the building, including
· Transportation from distribution center to construction site; initial on-site sorting of the materials;
· Wastage during distribution. · C2 transportation of the discarded product to a recycling site
and transportation of waste to final disposal;
A5: · C3 waste processing, collection of waste fractions from the
deconstruction and waste processing of material flows intended
· Installation process; for reuse, recycling and energy recovery;
· Transport of packaging waste to treatment site; · C4 waste disposal including physical pretreatment and
· Waste treatment of packaging. management of the disposal site.
The packaging material does not reach the end of waste state At the end of life, the MAGNA3 pump is manually disassembled
but is incinerated as waste. from the piping system in which it has been installed. The
According to European statistics, the average R1 value of definition of the applied end-of-life scenario in this EPD follows
incineration plants is > 0.6. Therefore, it is assumed the requirements in the
that packaging material is treated thermally in an incineration PCR Part A, 6.2 regarding complex products, with a
plant with R1 > 0.6. The loads from the combustion process of combination of recycling, thermal waste treatment and
packaging are declared in module A5 and the resulting energy landfilling. 100 % of the material is considered in the end of life
benefits in module D, as required by the PCR Part A, 5.5.2. scenario as required by the PCR. An overall collection rate of
90 % has been assumed.
Use stage (B1-B7):
Materials from which energy is recovered in an incineration
The use stage, related to the building fabric includes: process with an R1-value above 0.60 are in this study included
with the environmental burdens from the incineration process
· B1, use or application of the installed product; inventoried in C3, the recovered energy is declared as exported
· B2, maintenance. energy in C3
The use stage related to the operation of the building includes: and the energy benefits are declared in D. This procedure is
according to the PCR Part A, 5.5.6. C3 includes the mechanical
· B6, operational energy use; separation of the product followed by a series of sorting steps.
· B7, operational water use. Metal fractions are recycled and plastics, cardboard and
electronics are assumed incinerated with energy recovery. The
In this study, all use stage modules are assessed, though B1, residual fractions are landfilled and declared in C4.
B2 and B7 are assessed to be zero. By decision no. 20170712- The specific amounts are shown in the scenarios section.
n of the SVR, the modules B3, B4 and B5 are by default
declared as "MNR" (module Beyond system boundary (D): According to EN 15804
module D includes the reuse, recovery and/or recycling
not relevant). potentials, expressed as net impacts and benefits. Any
The modules include the provision and transport of all declared benefits and loads from net flows leaving the product
materials, products and related energy and water use, as well system that have not been allocated as co-products and that
as waste processing up to the end-of-waste state or disposal of have passed the end-of-waste state are included in module D.
final residues during the use stage. They also include all
4 Environmental Product Declaration - Grundfos Holding A/S - MAGNA3 100-40/60 (Cast Iron)
Contributions to module D comes from waste incineration lifespan: Europe
processes in A5 and C3 as well as material recycling in C3. The
specific fractions and net flows are shown in the scenarios
Comparability
section.
Basically, a comparison or an evaluation of EPD data is only
possible if all the data sets to be compared were created
according to EN 15804 and the building context, respectively
the product-specific characteristics of performance, are taken
Geographic Representativeness into account. Software and databases used: GaBi ts
Land or region, in which the declared product system is 9.2.1.68 (database schema 8007) Ecoinvent v3.5..
manufactured, used or handled at the end of the product´s
LCA: Scenarios and additional technical information
An estimated RSL of 10
Characteristic product properties of biogenic carbon years can be used to facilitate building calculations. This is an
The biogenic carbon content quantifies the amount of biogenic EU
carbon in a construction product leaving the factory gate, and it consensus-based estimation, referenced in Appendix 7: Lot 11
will be separately declared for the product and for any – Circulators in
accompanying packaging, as required from the PCR Part A. Buildings, prepared by AEA Energy & Environment for the
The Carbon content of Cardboard and Paper is assumed to European Commission
0.46 kg C. Overall, there is an amount of 9 weight-% Carbon in in the context of the Eco Design Directive
the product leaving the factory gate and has to be considered.
Reference service life
Name Value Unit
Information on describing the biogenic Carbon Content at
Life Span according to the manufacturer 10 a
factory gate
Name ValueUnit Operational energy use (B6)
Biogenic carbon content in accompanying 0.74 kg Name Value Unit
packaging C
Electricity consumption Group 1 1020 kWh/a
Note: 1 kg of biogenic carbon is equivalent to 44/12 kg of CO2 Electricity consumption Group 2 1285 kWh/a
Average power input, Group 1 0,204 kW
Average power input, Group 2 0,257 kW
The following technical scenario information is required for the
declared modules and optional for non-declared modules. Running hours (all groups) 5.000 h/a
Modules for which no information is declared can be deleted;
End of life (C1-C4)
additional information can also be listed if necessary.
Name Value Unit
The following technical information is a basis for the declared Collected as mixed construction waste 33,8 kg
modules or can be used for developing specific scenarios in the Transportation distance (C2) 500 km
context of a building assessment if modules are not declared
Aluminium for recycling 2,84 kg
(MND).
Steel for recycling 22,2 kg
A5 is not declared including the disposal of the packaging Copper for recycling 1,05 kg
material on the construction site, the amounts of packaging Stainless steel for recycling 1,09 kg
materials included in the LCA calculations must be declared as Plastics for incineration w/energy 1,58 kg
technical scenario information for Module A5.
Electronics for incineration w/energy 0,81 kg
Landfilling 4,23 kg
Transport from the gate to the site (A4) Reuse, recovery and/or recycling potentials (D), relevant
Name Value Unit scenario information
Litres of fuel 0,052 l/100km Name ValueUnit
Transport distance 2003 km A5, incineration w/energy recov. (LDPE foil) 6,19 MJ
Capacity utilisation (including empty runs) 85 % A5, incineration w/energy recov. (Paper/Cardboard) 11,2 MJ
Gross density of products transported 704 kg/m3 C3, steel for recycling (net amounts) -2,21 kg
Wastage during distribution 0,02 % C3, stainless steel for recycling (net amounts) 0,49 kg
C3, aluminium for recycling (net amounts) -0,39 kg
Installation into the building (A5)
C3, copper for recycling (net amounts) 0,451 kg
Name ValueUnit
C3, plastics for incineration, w/ energy recov. 1,58 kg
Packaging waste for incineration (LDPE film) 0,031 kg
C3, electronics for incineration, w/ energy recov. 0,81 kg
Packaging waste for incineration
2,81 kg
(Paper/Cardboard)
5 Environmental Product Declaration - Grundfos Holding A/S - MAGNA3 100-40/60 (Cast Iron)
LCA: Results
Characterization model: EN 15804 - 2012+A2 - 2019, PEF. By Decision no. 20170712-n of the IBU SVR, the modules B3, B4, B5 are
marked as MNR (module not relevant) as default. The LCA results in module B6 are given on a period of one year, according to PCR
Part B. To obtain the results from module B6 over the entire life cycle, the LCA results of module B6 must be multiplied by the
estimated RSL of 10 years. The indicator results for module B6 are declared for Group 1. B6 indicator results for other groups can be
derived by multiplying the B6 indicator results with the following factors:
Group 2: 1,259
DESCRIPTION OF THE SYSTEM BOUNDARY (X = INCLUDED IN LCA; ND = MODULE OR INDICATOR NOT DECLARED; MNR =
MODULE NOT RELEVANT)
Benefits and
Construction loads beyond
Product stage Use stage End of life stage
process stage the system
boundaries
la ire ta m w a Ry lp p u s tro p s n a rT g n iru tc a fu n a M e h t m o rf tro p s n a rTe tis e h t o t e ta g y lb m e s s A e s U e c n a n e tn ia M ria p e R tn e m e c a lp e R tn e m h s ib ru fe R y g re n e la n o ita re p Oe s u re ta w la n o ita re p Oe s u n o itc u rts n o c -e Dn o itilo m e d tro p s n a rT g n is s e c o rp e ts a W la s o p s iD -e s u e R-y re v o c e R-g n ilc y c e Rla itn e to p
A1 A2 A3 A4 A5 B1 B2 B3 B4 B5 B6 B7 C1 C2 C3 C4 D
X X X X X MND MND MNR MNR MNR X MND X X X X X
RESULTS OF THE LCA - ENVIRONMENTAL IMPACT according to EN 15804+A2: 1PCS of MAGNA3 100-40/60 (Cast Iron)
Parameter Unit A1 A2 A3 A4 A5 B6 C1 C2 C3 C4 D
GWP-total kg CO 2 eq 1.41E+02 2.12E+00 8.21E-02 2.28E+00 4.06E+00 4.13E+02 0 9.41E-01 8.39E+00 2.13E-01 1.49E-02
GWP-fossil kg CO 2 eq 1.4E+02 2.1E+00 4.84E+00 2.27E+00 1.86E-01 4.11E+02 0 9.35E-01 8.37E+00 2.19E-01 2.23E-02
GWP-
biogenic kg CO 2 eq 8.37E-01 -3.08E-03 -4.8E+00 -4.55E-03 3.88E+00 1.37E+00 0 -1.58E-03 1.02E-02 -6.61E-03 -2.45E-03
GWP-luluc kg CO 2 eq 2.82E-01 1.58E-02 4.23E-02 1.8E-02 1.38E-04 5.95E-01 0 7.6E-03 5.01E-03 1.93E-04 -4.96E-03
kg CFC11
ODP 1.04E-07 3.73E-16 4.08E-09 2.15E-11 7.41E-16 9.03E-12 0 1.72E-16 7.55E-14 4.93E-16 -7.88E-13
eq
AP mol H+ eq 6.48E-01 1.36E-02 1.91E-02 1.32E-02 1.17E-03 9.06E-01 0 5.52E-03 8.39E-03 6.81E-04 -2.13E-02
EP-
kg P eq 1.73E-03 5.99E-06 8.45E-05 7.15E-06 1.7E-07 1.1E-03 0 2.86E-06 1.33E-05 2.39E-05 -5.59E-06
freshwater
EP-marine kg N eq 8.84E-02 5.06E-03 4.09E-03 6.31E-03 4.29E-04 2.01E-01 0 2.66E-03 1.98E-03 1.57E-04 -3.25E-04
EP-terrestrial mol N eq 9.3E-01 5.61E-02 4.07E-02 6.99E-02 5.33E-03 2.12E+00 0 2.95E-02 2.18E-02 1.72E-03 -2.93E-03
kg NMVOC
POCP 2.77E-01 1.12E-02 1.14E-02 1.2E-02 1.12E-03 5.52E-01 0 5.06E-03 5.41E-03 5.05E-04 -1.29E-03
eq
ADPE kg Sb eq 7.51E-03 1.62E-07 6.1E-05 1.7E-06 1.24E-08 1.19E-04 0 7.6E-08 9.95E-07 1.48E-08 -1.26E-03
ADPF MJ 1.88E+03 2.8E+01 6.68E+01 3.05E+01 1.4E+00 7.22E+03 0 1.25E+01 6.14E+01 3.14E+00 -2.49E+01
m3 world eq
WDP 2.84E+01 1.93E-02 4.55E-01 2.94E-02 5.01E-01 8.95E+01 0 9.16E-03 1.24E+00 -2.42E-03 -9.93E-01
deprived
GWP = Global warming potential; ODP = Depletion potential of the stratospheric ozone layer; AP = Acidification potential of land and water; EP =
Eutrophication potential; POCP = Formation potential of tropospheric ozone photochemical oxidants; ADPE = Abiotic depletion potential for non-fossil
resources; ADPF = Abiotic depletion potential for fossil resources; WDP = Water (user) deprivation potential)
RESULTS OF THE LCA - INDICATORS TO DESCRIBE RESOURCE USE according to EN 15804+A2: 1PCS of MAGNA3 100-
40/60 (Cast Iron)
Parameter Unit A1 A2 A3 A4 A5 B6 C1 C2 C3 C4 D
PERE MJ 5.58E+02 1.51E+00 7.07E+01 1.9E+00 2.41E-01 3.2E+03 0 7.25E-01 2.67E+01 2.21E-01 -2.9E-01
PERM MJ 0 0 0 0 0 0 0 0 0 0 0
PERT MJ 5.58E+02 1.51E+00 7.07E+01 1.9E+00 2.41E-01 3.2E+03 0 7.25E-01 2.67E+01 2.21E-01 -2.9E-01
PENRE MJ 1.88E+03 2.81E+01 6.68E+01 3.06E+01 1.4E+00 7.22E+03 0 1.26E+01 6.14E+01 3.15E+00 -2.47E+01
PENRM MJ 0 0 0 0 0 0 0 0 0 0 0
PENRT MJ 1.88E+03 2.81E+01 6.68E+01 3.06E+01 1.4E+00 7.22E+03 0 1.26E+01 6.14E+01 3.15E+00 -2.47E+01
SM kg 2.88E+01 0 2.38E-01 5.8E-03 0 0 0 0 0 0 0
RSF MJ 1.46E-23 0 0 2.91E-27 0 0 0 0 0 0 0
NRSF MJ 1.71E-22 0 0 3.42E-26 0 0 0 0 0 0 0
FW m3 9.43E-01 1.77E-03 3.65E-02 2.27E-03 1.18E-02 3.7E+00 0 8.44E-04 4.23E-02 4E-05 1.61E-02
PERE = Use of renewable primary energy excluding renewable primary energy resources used as raw materials; PERM = Use of renewable primary
energy resources used as raw materials; PERT = Total use of renewable primary energy resources; PENRE = Use of non-renewable primary energy
excluding non-renewable primary energy resources used as raw materials; PENRM = Use of non-renewable primary energy resources used as raw
materials; PENRT = Total use of non-renewable primary energy resources; SM = Use of secondary material; RSF = Use of renewable secondary fuels;
NRSF = Use of non-renewable secondary fuels; FW = Use of net fresh water
RESULTS OF THE LCA – WASTE CATEGORIES AND OUTPUT FLOWS according to EN 15804+A2:
1PCS of MAGNA3 100-40/60 (Cast Iron)
6 Environmental Product Declaration - Grundfos Holding A/S - MAGNA3 100-40/60 (Cast Iron)
Parameter Unit A1 A2 A3 A4 A5 B6 C1 C2 C3 C4 D
HWD kg 5.79E-04 1.21E-06 1.22E-04 1.22E-04 1.51E-06 2.99E-06 0 5.82E-07 2.96E-08 1.26E-08 -3.09E-04
NHWD kg 5.5E+00 4.34E-03 3.2E-01 6.24E-03 1.32E-01 5.12E+00 0 1.99E-03 8.75E-01 3.6E+00 1.96E+00
RWD kg 8.67E-02 5.04E-05 1.83E-03 8.06E-05 6.75E-05 1.1E+00 0 2.32E-05 9.13E-03 3.77E-05 -2.66E-03
CRU kg 0 0 0 0 0 0 0 0 0 0 0
MFR kg 0 0 0 0 0 0 0 0 2.72E+01 0 0
MER kg 0 0 0 0 0 0 0 0 0 0 0
EEE MJ 0 0 0 0 6.19E+00 0 0 0 8.26E+00 0 0
EET MJ 0 0 0 0 1.12E+01 0 0 0 1.49E+01 0 0
HWD = Hazardous waste disposed; NHWD = Non-hazardous waste disposed; RWD = Radioactive waste disposed; CRU = Components for re-use;
MFR = Materials for recycling; MER = Materials for energy recovery; EEE = Exported electrical energy; EET = Exported thermal energy
RESULTS OF THE LCA – additional impact categories according to EN 15804+A2-optional:
1PCS of MAGNA3 100-40/60 (Cast Iron)
Parameter Unit A1 A2 A3 A4 A5 B6 C1 C2 C3 C4 D
Disease
PM 8.38E-06 1.44E-07 2.64E-07 7.82E-08 6.61E-09 7.6E-06 0 3.23E-08 7.07E-08 6.94E-09 -3.26E-07
incidence
IR kBq U235 eq 9.48E+00 7.42E-03 2.89E-01 1.13E-02 1.04E-02 1.8E+02 0 3.42E-03 1.5E+00 5.35E-03 -2.87E-01
ETP-fw CTUe 9.96E+02 2.08E+01 2.06E+01 2.24E+01 7.04E-01 3.09E+03 0 9.38E+00 2.66E+01 2.22E+00 -1.4E+01
HTP-c CTUh 1.67E-06 4.29E-10 6.61E-07 9.32E-10 3.45E-11 8.53E-08 0 1.94E-10 7.87E-10 1.27E-10 -6.23E-08
HTP-nc CTUh 2.91E-06 2.36E-08 6.59E-08 2.7E-08 1.59E-09 3.14E-06 0 1.11E-08 3.12E-08 1.11E-08 -1.2E-08
SQP SQP 5.7E+02 9.16E+00 1.39E+02 1.06E+01 3.81E-01 2.3E+03 0 4.4E+00 1.94E+01 2.27E-01 -2.69E+01
PM = Potential incidence of disease due to PM emissions; IR = Potential Human exposure efficiency relative to U235; ETP-fw = Potential comparative
Toxic Unit for ecosystems; HTP-c = Potential comparative Toxic Unit for humans (cancerogenic); HTP-nc = Potential comparative Toxic Unit for humans
(not cancerogenic); SQP = Potential soil quality index
Disclaimer 1 – for the indicator 'Potential Human exposure efficiency relative to U235'.
This impact category deals mainly with the eventual impact of low-dose ionizing radiation on human health of the nuclear fuel cycle. It
does not consider effects due to possible nuclear accidents, occupational exposure, or radioactive waste disposal in underground
facilities. Potential ionizing radiation from the soil, radon and some construction materials is also not measured by this indicator.
Disclaimer 2 – for the indicators 'abiotic depletion potential for non-fossil resources', 'abiotic depletion potential for fossil resources',
'water (user) deprivation potential, deprivation-weighted water consumption', 'potential comparative toxic unit for ecosystems', 'potential
comparative toxic unit for humans – cancerogenic', 'Potential comparative toxic unit for humans - not cancerogenic', 'potential soil
quality index'. The results of this environmental impact indicator shall be used with care, as the uncertainties on these results are high
or as there is limited experience with the indicator.
Disclaimer 3: JRC Technical Reports, Version 2, 2018 Page 6, for the indicator "EP-freshwater". This indicator has been calculated as
'kg P eq' as required in the characterization model EUTREND model, Struijs et al., 2009b, as implemented in ReCiPe; This EPD was
created using a software tool.
References
Standards
Ecodesign Directive
Machinery Directive
DIRECTIVE 2009/125/EC OF THE EUROPEAN
DIRECTIVE 2006/42/EC OF THE EUROPEAN
PARLIAMENT AND OF THE COUNCIL of 21 October
PARLIAMENT AND OF THE COUNCIL of 17 May
2009 establishing a framework for the setting of
2006 on machinery
eco-design requirements for energy-related products
Radio Equipment Directive
DIRECTIVE 2014/53/EU OF THE EUROPEAN PARLIAMENT
AND OF THE COUNCIL of 16 April 2014 on the harmonization EC 641/2009
of the laws of the Member States relating to the making
available on the market of radio equipment COMMISSION REGULATION (EC) No 641/2009 of 22 July
2009 implementing Directive 2005/32/EC of the European
Parliament and of the Council with regard to eco-design
Electromagnetic Compatibility (EMC) Directive requirements for glandless standalone circulators and
glandless circulators integrated in products
DIRECTIVE 2014/30/EU OF THE EUROPEAN
PARLIAMENT AND OF THE COUNCIL of 26 February
EC 622/2012
2014 on the harmonization of the laws of the Member
COMMISSION REGULATION (EU) No 622/2012 of 11 July
States relating to electromagnetic compatibility 2012 amending Regulation (EC) No 641/2009 with regard to
eco-design requirements for glandless standalone circulators
7 Environmental Product Declaration - Grundfos Holding A/S - MAGNA3 100-40/60 (Cast Iron)
and glandless circulators integrated in products
EN 50581:2012
DIRECTIVE 2011/65/EU
EN 50581:2012, Technical documentation for the
DIRECTIVE 2011/65/EU OF THE EUROPEAN
assessment of electrical and electronic products with
PARLIAMENT AND OF THE COUNCIL of 8 June 2011
respect to the restriction of hazardous substances
on the restriction of the use of certain hazardous
substances in electrical and electronic equipment
EN 60335-1
DIRECTIVE 2015/863/EU EN 60335-1:2012/A11:2014/A13:2017, Household
DIRECTIVE 2015/863/EU of 31 March 2015 amending and similar electrical appliances – Safety – Part 1: General
requirements
Annex II to Directive 2011/65/EU of the European
Parliament and of the Council as regards the list of
EN 60335-2-51
restricted substances
EN 60335-2-51:2003-03 + A1:2008 + A2:2012, Household and
similar electrical appliances – Safety –Part 2-51: Particular
ETSI EN 301 489-1 requirements for stationary circulation pumps for heating and
service water installations
ETSI EN 301 489-1 V2.2.0, Electromagnetic Compatibility
(EMC) standard for radio equipment and services; Part 1:
Common technical requirements
EN 61000-3-2
ETSI EN 301 489-17 EN 61000-3-2:2014/2019, Electromagnetic compatibility (EMC)
– Part 3-2: Limits – Limits for harmonic current emissions
ETSI EN 301 489-17 V3.2.0, Electromagnetic Compatibility (equipment input current =16 A per phase)
(EMC) standard for radio equipment and services; Part 17:
Specific conditions for Broadband Data Transmission Systems
EN 61000-3-3
ETSI EN 300 328 V2.1.1
EN 61000-3-3:2013-08/ A1:2019, Electromagnetic compatibility
ETSI EN 300 328 V2.1.1, Wideband transmission systems; (EMC) – Part 3-3:
Data transmission equipment operating in the 2,4 GHz ISM Limits – Limitation of voltage changes, voltage fluctuations and
band and using wide band modulation techniques flicker in public low voltage supply systems, for equipment with
rated current <= 16 A per phase and not subject to conditional
EN 809 connection
EN 809:1998-10 + A1:2009, Pumps and pump units for
liquids - Common safety requirements EN 61000-6-2
EN 55014-1 EN 61000-6-2:2008/2019, Electromagnetic compatibility (EMC)
– Part 6-2: Generic standards –Immunity for industrial
EN 55014-1:2017, Electromagnetic compatibility – environments
Requirements for household appliances, electric tools and
similar apparatus – Part 1: Emission EN 16297-1
EN 16297-1:2012-10, Pumps – Rotodynamic pumps –
Glandless circulators – Part 1:
EN 55014-2 General requirements and procedures for testing and
calculation of energy efficiency index (EEI)
EN 55014-2:2015, Electromagnetic compatibility –
EN 16297-2
Requirements for household appliances, electric tools
EN 16297-2:2012-10, Pumps – Rotodynamic pumps –
and similar apparatus – Part 2: Immunity – Product Glandless circulators – Part 2: Calculation of energy efficiency
index (EEI) for standalone circulators
family standard (CISPR 14-2:2015)
8 Environmental Product Declaration - Grundfos Holding A/S - MAGNA3 100-40/60 (Cast Iron)
EN 16297-3
CPR
EN 16297-3:2012, Pumps – Rotodynamic pumps –Glandless REGULATION (EU) No 305/2011 OF THE EUROPEAN
circulators – Part 3: Energy efficiency index (EEI) for circulators PARLIAMENT AND OF THE COUNCIL of 9 March 2011 laying
integrated in products down harmonized conditions for the marketing of construction
products and repealing Council Directive 89/106/EEC
CML 2001
ISO 14001 Impact assessment characterization factors Institute of
Environmental Sciences, Leiden University, Netherlands
EN ISO 14001:2015-09, Environmental management systems - ECHA candidate list
Requirements with guidance for use Candidate List of substances of very high concern (SVHCs) for
authorization, European Chemicals Agency (ECHA), Helsinki,
Finland
ISO 14025
Ecoinvent
DIN EN /ISO 14025:2011-10, Environmental labels and Ecoinvent v3.5
declarations — Type III environmental declarations —
Principles and procedures GaBi ts
GaBi ts 9.2.1.68 (database schema 8007)
REACH
EN 15804
Regulation (EC) No 1907/2006 of the European Parliament and
EN 15804:2012-04+A1 2013, Sustainability of construction of the Council of 18 December 2006 concerning the
works — Environmental Product Declarations — Core rules for Registration, Evaluation, Authorization and Restriction of
the product category of construction products Chemicals (REACH) (Status: 27.06.2018)
PCR Part A SVR
Advisory Board (formerly SVA) Decision no. 20170712-n
Institut Bauen und Umwelt e.V., Berlin (pub.): Product Category
Rules for Building-Related Products and Services, Product The literature referred to in the Environmental Product
Category Rules for Construction Products from the range of Declaration must be listed in full.
Environmental Product Declarations of Institut Bauen und
Umwelt (IBU), Part A: Calculation Rules for the Life Cycle Standards already fully quoted in the EPD do not need to be
Assessment and Requirements on the Project Report, Version listed here again.
1.7 (2021)
The current version of PCR Part A and PCR Part B of the PCR
document on which they are based must be referenced. The
literature referred to in the Environmental Product Declaration
PCR Part B must be listed in full.
Institut Bauen und Umwelt e.V., Berlin (pub.): Product Category
Rules for Building-Related Products and Services, Product
Category Rules for Construction Products from the range of Standards already fully quoted in the EPD do not need to be
Environmental Product Declarations of Institut Bauen und listed here again.
Umwelt (IBU), Part B: Requirements on the EPD for Pumps for
liquids and liquids with solids, Version 1.0 (2018) The current version of PCR Part A and PCR Part B of the PCR
document on which they are based must be referenced
.
The literature referred to in the Environmental Product
Declaration must be listed in full.Standards already fully quoted
in the EPD do not need to be listed here again.
The current version of PCR Part A and PCR Part B of the PCR
document on which they are based must be referenced.
Further references
9 Environmental Product Declaration - Grundfos Holding A/S - MAGNA3 100-40/60 (Cast Iron)
Publisher
Institut Bauen und Umwelt e.V. +49 (0)30 3087748- 0
Hegelplatz 1 info@ibu-epd.com
10117 Berlin www.ibu-epd.com
Germany
Programme holder
Institut Bauen und Umwelt e.V. +49 (0)30 3087748- 0
Hegelplatz 1 info@ibu-epd.com
10117 Berlin www.ibu-epd.com
Germany
Author of the Life Cycle Assessment
Grundfos Holding A/S +45 87501400
Poul Due Jensens Vej 7 atomic@grundfos.com
8850 Bjerringbro www.grundfos.com
Denmark
Owner of the Declaration
Grundfos Holding A/S +45 87501400
Poul Due Jensens Vej 7 atomic@grundfos.com
8850 Bjerringbro www.grundfos.com
Denmark
10 Environmental Product Declaration - Grundfos Holding A/S - MAGNA3 100-40/60 (Cast Iron)
