ENVIRONMENTAL PRODUCT DECLARATION
as per ISO 14025 and EN 15804+A2
Owner of the Declaration Grundfos Holding A/S
Publisher Institut Bauen und Umwelt e.V. (IBU)
Programme holder Institut Bauen und Umwelt e.V. (IBU)
Declaration number EPD-GRU-20230076-CBC1-EN
Issue date 21.11.2023
Valid to 20.11.2028
MAGNA3 40-120/150/180 (Cast Iron)
Grundfos Holding A/S
www.ibu-epd.com | https://epd-online.com
General Information
Grundfos Holding A/S MAGNA3 40-120/150/180 (Cast Iron)
Programme holder Owner of the declaration
IBU – Institut Bauen und Umwelt e.V. Grundfos Holding A/S
Hegelplatz 1 Poul Due Jensens Vej 7
10117 Berlin 8850 Bjerringbro
Germany Denmark
Declaration number Declared product / declared unit
EPD-GRU-20230076-CBC1-EN 1 PCS. of MAGNA3 40-120/150/180 (Cast Iron)
This declaration is based on the product category rules: Scope:
Pumps for liquids and liquids with solids, 01.08.2021 The declaration applies to 1 piece of MAGNA3 (Cast Iron) pump.
(PCR checked and approved by the SVR)
The product is produced in Wahlstedt, Germany, and the life cycle
assessment is based on data collected at the production site. Production
Issue date has been modeled using annual production data from 2021. The
declaration covers three different types of the MAGNA3 40- product
21.11.2023
(120/150/180).
The owner of the declaration shall be liable for the underlying information
Valid to
and evidence; the IBU shall not be liable with respect to manufacturer
20.11.2028 information, life cycle assessment data and evidences.
The EPD was created according to the specifications of EN 15804+A2. In
the following, the standard will be simplified as EN 15804.
Verification
The standard EN 15804 serves as the core PCR
Independent verification of the declaration and data according to ISO
14025:2011
internally X externally
Dipl.-Ing. Hans Peters
(Chairman of Institut Bauen und Umwelt e.V.)
Florian Pronold Mrs Kim Allbury,
(Managing Director Institut Bauen und Umwelt e.V.) (Independent verifier)
1 Environmental Product Declaration - Grundfos Holding A/S - MAGNA3 40-120/150/180 (Cast Iron)
Product
EN 60335-1:2012/AC:2014 + A11:2014, EN 60335-2-51:2003 +
Product description/Product definition A1:2008 + A2:2012,
The Grundfos MAGNA3 circulator pumps are designed for EN 62233:2008.
circulating liquids in heating systems, air conditioning and
cooling systems and domestic hot water systems. However, the
pump range can also be used in ground source heat pump
systems and solar heating systems. EN 55014-1:2006
+ A1:2009 + A2:2011, EN 55014-1:2017, EN 61000-6-2:2005,
EN 61000-3-2:2014, EN
61000-3-3:2013, ETSI EN 301 489-1 V2.2.0, ETSI EN 301 489-
The MAGNA3 pump is a centrifugal pump powered by an 17 V3.2.0. ETSI EN
electrical motor. It has a high-performance neodymium magnet 300 328 V2.1.1
rotor which increases motor efficiency and an insulation shell to
reduce heat loss from the cast iron pump housing with threaded
connections.
The declaration covers three types of the MAGNA3 pump. They
are grouped as shown below. The group reference in the Electromagnetic
technical data and scenarios refers also to these. Compatibility (EMC) Directive (2014/30/EU)
GROUP 1 - MAGNA3 40-120 Standards used:
EN 55014-1:2017, EN 55014-2:2015,
GROUP 2 - MAGNA3 40-150 GROUP 3 - MAGNA3 40-180
These are all the same physical products and 100 % identical
in terms of design, dimensions and materials as well as supply
chain and manufacturing processes, i.e., all cradle to gate EN
processes (A1-A3). 61000-3-2:2014/2019, EN 61000-6-2:2008/2019,
The products are also identical in terms of packaging,
distribution, reference service life and end-of-life treatment. The
only thing that differentiates the products from each other is the EN
software which controls how the pump operates in the system 61000-3-3:2013 A1:2019
in which it is installed, making them fit for different applications.
Hence, all life cycle modules are identical, except use stage
module B6, which will change, as the applied scenarios for
electricity consumption changes. For the placing
on the market in the European Union/European Free Trade
Association (EU/EFTA) (with the exception of Switzerland) the
following
legal provisions apply: RoHS Directive
2011/65/EU and 2015/863//EU
Machinery
Directive (2006/42/EC) Standard: EN
50581:2012.
Standard used: EN
809:1998 + A1:2009.
Ecodesign
Directive (2009/125/EC)
Radio Equipment
Directive (2014/53/EU) Commission
Regulation (EC) No: 641/2009 and
Standards used:
2 Environmental Product Declaration - Grundfos Holding A/S - MAGNA3 40-120/150/180 (Cast Iron)
Commission Others are given
Regulation (EU) 622/2012 individually for all two groups.
Standards used:
Constructional data
EN 16297-1:2012, EN 16297-2:2012, EN 16297-3:2012.
Name Value Unit
Frequency 50 Hz
Voltage 230 V
nominal capacity - kW
Clean
Pumped liquid (e.g. water) -
Water
Energy Efficiency Index Gr.1 0,18
The CE marking takes into account the proof of conformity with
the respective harmonized norms based on the legal provisions Energy Efficiency Index Gr.2 0,17
above. Energy Efficiency Index Gr.3 0,17
Flow range Gr. 1 (max) 23,0 m3/h
Flow range Gr. 2 (max) 25,0 m3/h
MAGNA3 pumps Flow range Gr. 3 (max) 25,0 m3/h
are not harmonized in accordance with the CPR. Head max. Gr.1 12 m
Head max. Gr.2 15 m
Application
Head max. Gr.3 18 m
For the application and use the respective national
Power input Gr. 1 Average (from load profile
0,179 kW
provisions apply. describing use)
Power input Gr. 2 Average (from load profile
0,252 kW
The pump is designed for circulating liquids in the describing use)
Power input Gr. 3 Average (from load profile
0,252 kW
following systems: describing use)
Nominal capacity Gr.1 0,427 kW
· heating systems
Nominal capacity Gr. 2 0,608 kW
Nominal capacity Gr.3 0,609 kW
· domestic hot-water systems
Performance
· air-conditioning and cooling systems data of the product according to the harmonized
standards, based on provisions for harmonization.
· ground-source heat-pump systems
Base materials/Ancillary materials
· solar-heating systems
Base materials / Ancillary materials
Name Value Unit
The pump is suitable for thin, clean, non-aggressive and non-
explosive liquids, not containing solid particles or fibres that Aluminium 17 %
may attack the pump mechanically or chemically. In heating Cast iron 45 %
systems, the water must meet the requirements of accepted Ceramics 0,4 %
standards on water quality in heating systems. The pumps are
Copper 3 %
also suitable for domestic hot-water systems.
Electronics 0,3 %
Technical Data Magnet Nd 1 %
The performance Paper 1 %
data of the product according to the harmonized norms, based PCB 5 %
on the
Plastics 0,4 %
harmonization provisions above apply.
Plastics, foam 1 %
Plastics GF 7 %
Rubber 0,2 %
The relevant Stainless steel 5 %
technical specifications according to the PCR Part B are given
Steel 6 %
in
Cardboard 7 %
the table below.
Plastic film 0,1 %
TOTAL 100 %
REACH
Characteristics
that are the same for all product groups are only given once.
3 Environmental Product Declaration - Grundfos Holding A/S - MAGNA3 40-120/150/180 (Cast Iron)
This product/article/at least one partial article
contains
There is no definitive information on the average circulator
life available, there is consensus within the industry that it is at
least 12
substances listed in the ECHA candidate list (date: years. However, this is complicated by many factors, including
many being
scrapped prematurely when e.g. the boiler they are connected
to is
10.06.2022) exceeding 0.1 percentage by mass: no replaced.
The Wahlstedt production has been assessed and From the estimated stock (140Mpa) and annual
certified as meeting the requirements in ISO 14001, ISO 50001, sales (14Mpa), the average lifetime of the circulator is taken as
ISO 10 years for the purposes of this study.
45001 and ISO 9001.
Reference service life
No use stage scenario which refers to the lifetime of
the product is declared. However, to facilitate building
calculations, an
estimated RSL of 10 years can be used. This is an EU
consensus-based The RSL of the declared product is not directly
estimation, referenced on page 37 in Appendix 7: Lot 11 – influencing the results in this study, as no declared use stage
Circulators in scenario is
Buildings, prepared by AEA Energy & Environment for the dependent on the RSL; The use stage sub-module B6 is
European declared per year as
Commission in the context of the Eco Design Directive: required by the PCR Part B.
LCA: Calculation rules
Declared Unit
The declared unit is 1 piece (pcs.) of MAGNA3 (Cast
iron) pump.
Declared unit
Name Value Unit
Declared unit 1 pce.
The product stage (A1-A3)
Mass reference 18.06 kg/pce comprises raw material extraction and processing, transport
Conversion factor [Mass/Declared Unit] 18.06 processes as well
as the manufacturing process. The final production and
For IBU core EPDs (where clause 3.6 is part of the EPD): for
assembly of the MAGNA3
average EPDs, an estimate of the robustness of the LCA
pump takes place at a Grundfos manufacturing site in
values must be made, e.g. concerning the variability of the
Germany. However, the full
production process, geographical representativeness and the
supply-chain leading to the finished product at the gate is rather
influence of background data and preliminary products
complex and
compared to the environmental impacts caused by the actual
includes a large amount of raw materials, components and
production.
semi-finished parts
which comes from both external suppliers as well as other
System boundary Grundfos production
facilities.
This EPD is Cradle-To-Grave. The system boundaries
of the EPD follow the modular approach in EN 15804.
By decision no. 20170712-n of the SVR, the modules B3, B4
and B5 are by
default declared as "MNR" (module not relevant).
4 Environmental Product Declaration - Grundfos Holding A/S - MAGNA3 40-120/150/180 (Cast Iron)
· A3
Manufacturing of packaging;
The product stage is included in the study, and
according to EN 15804 the system boundary with nature is set
to include
those processes that provide the material and energy inputs · A1-A3
into the system and the following manufacturing, transport up to processing up to the end-of-waste state or disposal of final
the factory residues.
gate as well as the processing any waste arising from those
processes.
For secondary material inputs, the system boundary to
the previous system (providing the secondary material) is set
Wastes and losses are included in the modules where where outputs
they occur according to the polluter pays principle and the reach the end-of-waste state. The recycling of secondary
modular approach of material into new raw
EN 15804. materials is included in the system boundary of this study.
Waste
materials from production processes that are recycled
without any modification of the material's inherent
characteristics are modelled
The product includes: as closed-loop within A1-A3. This is done up to the input mass
flow that was
used during production.
· A1
Extraction and processing of raw materials;
· A1 Reuse
of products or materials from a previous product system; Waste for incineration arising in the product stage is
accounted for in the module where the waste is produced. The
environmental
loads from the incineration process are declared in the module
· A1 where it occurs
Processing of secondary materials; and the electricity and heat which are produced from the
incineration is
considered as closed-loop within A1-A3, as described in PCR
Part A,
· A1 5.5.1. The input of biogenic carbon from the production of
Generation of electricity, steam and heat from primary energy packaging material is
resources, also inventoried in A3. As required by PCR Part A, the
including their extraction, refining and transport; corresponding
end-of-life module of the packaging material, A5, is also
declared and the
emissions of biogenic carbon are inventoried.
· A1 Energy
recovery and other recovery processes from secondary fuels;
· A2
Transportation up to the factory gate and internal transport;
The construction process stage (A4-A5) includes:
· A3
Production of ancillary materials or pre products; A4:
· A3 Manufacturing ·
of products and coproducts; Transportation from factory gate to distribution center:
5 Environmental Product Declaration - Grundfos Holding A/S - MAGNA3 40-120/150/180 (Cast Iron)
·
Consumption of electricity, thermal energy and water at
distribution center; · B1, use or
application of the installed product;
·
Transportation from distribution center to construction site; · B2,
maintenance.
· Wastage
during distribution. The use stage related to the operation of the building
A5: includes:
· · B6,
Installation process; operational energy use;
· Transport · B7,
of packaging waste to treatment site; operational water use.
· Waste In this study, all use stage modules are assessed,
treatment of packaging. though B1, B2 and B7 are assessed to be zero. By decision no.
20170712-n of the
SVR, the modules B3, B4 and B5 are by default declared as
"MNR" (module
The packaging material does not reach the end of waste
state but is incinerated as waste. According to European
statistics, the
average R1 value of incineration plants is > 0.6. Therefore, it is not relevant). The modules include the provision and
assumed transport of all materials, products and related energy and
water use, as well
as waste processing up to the end-of-waste state or disposal of
final residues
that packaging material is treated thermally in an during the use stage. They also include all impacts and
incineration plant with R1 > 0.6. The loads from the combustion
process of
packaging are declared in module A5 and the resulting energy
benefits in module aspects related to the losses during the use stage
(i.e. production, transport, and waste processing and disposal
of the lost
products and materials).
D, as required by the PCR Part A, 5.5.2.
Generally, the geographical coverage of the datasets
Use stage (B1-B7): used matches the actual processes taking place. Meaning, that
when modelling
taking place in Grundfos Bjerringbro, the Danish electricity grid
mix is used
in the model and thermal energy from natural gas. These are
generally
of very high quality with very good technological, temporal and
geographical
The use stage, related to the building fabric representativeness.
includes:
6 Environmental Product Declaration - Grundfos Holding A/S - MAGNA3 40-120/150/180 (Cast Iron)
energy recovery;
· C4 waste
disposal including physical pretreatment and management of
Contributions to operational energy use during the use the disposal site.
stage (B6) come from the electricity consumption of the
product. The annual
electricity consumption is calculated by multiplying the average
power input, At the end of life, the MAGNA3 pump is manually
which is based on a defined load profile, with the annual disassembled from the piping system in which it has been
running hours. installed. The
For use stage (B6) European Average electricity grid mix has definition of the applied end-of-life scenario in this EPD follows
been used. These the
values are declared in the scenarios section. requirements in the
PCR Part A, 6.2 regarding complex products,
with a combination of recycling, thermal waste treatment and
landfilling. 100 %
of the material is considered in the end of life scenario as
The End-of-Life stage (C1-C4) required by the PCR.
includes all activities from when the product reaches the end of An overall collection rate of 90 % has been assumed.
its service
life and no longer provides any functionality and until all
materials and
components are processed for
reuse/recycling or disposed of. Materials from which energy is recovered in an
incineration process with an R1-value above 0.60 are in this
study included with
the environmental burdens from the incineration process
inventoried in C3, the
recovered energy is declared as exported energy in C3
According to EN 15804 and the PCR Part A,
the end-of-life stage includes: and the energy benefits are declared in D. This
procedure is according to the PCR Part A, 5.5.6. C3 includes
the
mechanical separation of the product followed by a series of
· C1 sorting steps.
deconstruction of the product from the Metal fractions are recycled and plastics, cardboard and
electronics are
assumed incinerated with energy recovery. The residual
fractions are landfilled
· building, and declared in C4.
including initial on-site sorting of the
The specific amounts are shown in the scenarios section.
· materials;
· C2
transportation of the discarded product to a recycling site and
transportation
of waste to final disposal; Beyond system boundary (D):
According to EN 15804 module D includes the reuse, recovery
and/or
recycling potentials, expressed as net impacts and benefits.
· C3 waste Any declared
processing, collection of waste fractions from the benefits and loads from net
deconstruction and waste
processing of material flows intended for reuse, recycling and
7 Environmental Product Declaration - Grundfos Holding A/S - MAGNA3 40-120/150/180 (Cast Iron)
flows leaving the product system that have not been Comparability
allocated as co-products and that have passed the end-of- Basically, a comparison or an evaluation of EPD data is only
waste state are possible if all the data sets to be compared were created
included in module D. according to EN 15804 and the building context, respectively
the product-specific characteristics of performance, are taken
into account. Software and databases used: GaBi ts
Contributions to module D comes from waste
incineration processes in A5 and C3 as well as material
recycling in C3. The 9.2.1.68
specific fractions and net flows are shown in the scenarios (database schema 8007) Ecoinvent v3.5..
section.
Geographic Representativeness
Land or region, in which the declared product system is
manufactured, used or handled at the end of the product´s
lifespan: Europe
LCA: Scenarios and additional technical information
Name Value Unit
Characteristic product properties of biogenic carbon
Litres of fuel 0,052 l/100km
The
Transport distance 2003 km
biogenic carbon content quantifies the amount of biogenic
carbon in a Capacity utilisation (including empty runs) 85 %
construction product leaving the factory gate, and it will be Gross density of products transported 347 kg/m3
separately
Wastage during distribution 0,02 %
declared for the product and for any accompanying packaging,
as required from Installation into the building (A5)
the PCR Part A. The Carbon content of Cardboard and Paper is
Name ValueUnit
assumed to
Packaging waste for incineration (LDPE film) 0,031 kg
0.46 kg C. Overall, there is an amount of 9 weight-% Carbon in
the product Packaging waste for incineration 1,42 kg
leaving the factory gate and has to be considered (Paper/Cardboard)
An
estimated RSL of 10 years can be used to facilitate building
calculations. This
is an EU consensus-based estimation, referenced in Appendix
Information on describing the biogenic Carbon Content at 7: Lot 11 –
factory gate Circulators in Buildings, prepared by AEA Energy &
Environment for the
Name ValueUnit
European Commission in the context of the Eco Design
Biogenic carbon content in accompanying kg
0.74 Directive.
packaging C
Reference service life
Note: 1 kg of biogenic carbon is equivalent to 44/12 kg of CO2
Name Value Unit
Life Span according to the manufacturer 10 a
The following technical scenario information is required for the
Operational energy use (B6)
declared modules and optional for non-declared modules.
Modules for which no information is declared can be deleted; Name Value Unit
additional information can also be listed if necessary. Electricity consumption, Group 1 895 kWh/a
Electricity consumption, Group 2 1260 kWh/a
The following technical information is a basis for the declared
Electricity consumption, Group 3 1260 kWh/a
modules or can be used for developing specific scenarios in the
Average power input, Group 1 0,179 kW
context of a building assessment if modules are not declared
(MND). Average power input, Group 2 0,252 kW
Average power input, Group 3 0,252 kW
A5 is not declared including the disposal of the packaging
Running hours (all groups) 5.000 h/a
material on the construction site, the amounts of packaging
materials included in the LCA calculations must be declared as End of life (C1-C4)
technical scenario information for Module A5.
Transport from the gate to the site (A4)
8 Environmental Product Declaration - Grundfos Holding A/S - MAGNA3 40-120/150/180 (Cast Iron)
Name Value Unit Reuse, recovery and/or recycling potentials (D), relevant
Collected as mixed construction waste 16,77 kg scenario information
Transportation distance (C2) 500 km Name Value Unit
Aluminium for recycling 2,79 kg A5, incineration w/energy recov. (LDPE foil) 3,21 MJ
Steel for recycling 8,19 kg A5, incineration w/energy recov.
5,82 MJ
Copper for recycling 0,51 kg (Paper/Cardboard)
Stainless steel for recycling 0,82 kg C3, steel for recycling (net amounts) -0,935 kg
Plastics for incineration w/energy 1,28 kg C3, stainless steel for recycling (net amounts) 0,53 kg
Electronics for incineration w/energy 0,81 kg C3, aluminium for recycling (net amounts) -0,383 kg
Landfilling 1,89 kg C3, copper for recycling (net amounts) 0,221 kg
C3, plastics for incineration, w/ energy recov. 1,28 kg
C3, electronics for incineration, w/ energy recov. 0,814 kg
9 Environmental Product Declaration - Grundfos Holding A/S - MAGNA3 40-120/150/180 (Cast Iron)
LCA: Results
Characterization model: EN 15804 - 2012+A2 -
2019, PEF. By Decision no. 20170712-n of the IBU SVR, the modules B3, B4, B5
are marked as MNR (module not relevant) as default. The LCA results in module
B6 are given on a period of one year, according to PCR Part B. To obtain
the results from module B6 over the entire life cycle, the LCA results of
module B6 must be multiplied by the estimated RSL of 10 years. The
indicator results for module B6 are declared for Group 1. B6 indicator results
for other groups can be derived by multiplying the B6 indicator results with
the following factors:
Group 2: 1,37
Group 3: 1,37
DESCRIPTION OF THE SYSTEM BOUNDARY (X = INCLUDED IN LCA; ND = MODULE OR INDICATOR NOT DECLARED; MNR =
MODULE NOT RELEVANT)
Benefits and
Construction loads beyond
Product stage Use stage End of life stage
process stage the system
boundaries
la ire ta m w a Ry lp p u s tro p s n a rT g n iru tc a fu n a M e h t m o rf tro p s n a rTe tis e h t o t e ta g y lb m e s s A e s U e c n a n e tn ia M ria p e R tn e m e c a lp e R tn e m h s ib ru fe R y g re n e la n o ita re p Oe s u re ta w la n o ita re p Oe s u n o itc u rts n o c -e Dn o itilo m e d tro p s n a rT g n is s e c o rp e ts a W la s o p s iD -e s u e R-y re v o c e R-g n ilc y c e Rla itn e to p
A1 A2 A3 A4 A5 B1 B2 B3 B4 B5 B6 B7 C1 C2 C3 C4 D
X X X X X MND MND MNR MNR MNR X MND X X X X X
RESULTS OF THE LCA - ENVIRONMENTAL IMPACT according to EN 15804+A2: 1PCS of MAGNA3 40-120/150/180 (Cast Iron)
Parameter Unit A1 A2 A3 A4 A5 B6 C1 C2 C3 C4 D
GWP-total kg CO 2 eq 9.2E+01 1.15E+00 1.3E+00 1.13E+00 2.09E+00 3.62E+02 0 4.63E-01 5.81E+00 1.12E-01 -4.09E-01
GWP-fossil kg CO 2 eq 9.15E+01 1.15E+00 3.59E+00 1.12E+00 1.32E-01 3.6E+02 0 4.6E-01 5.8E+00 1.15E-01 -4.05E-01
GWP-
biogenic kg CO 2 eq 2.89E-01 -1.47E-03 -2.32E+00 -2.26E-03 1.96E+00 1.2E+00 0 -7.76E-04 4.96E-03 -3.46E-03 -1.93E-03
GWP-luluc kg CO 2 eq 1.37E-01 8.07E-03 3.3E-02 8.88E-03 7.12E-05 5.22E-01 0 3.74E-03 2.49E-03 1.01E-04 -2.48E-03
kg CFC11
ODP 9.14E-08 1.97E-16 4.06E-09 1.91E-11 3.85E-16 7.93E-12 0 8.48E-17 3.74E-14 2.59E-16 -7.53E-13
eq
AP mol H+ eq 5.36E-01 9.54E-03 1.59E-02 6.55E-03 5.99E-04 7.95E-01 0 2.72E-03 4.44E-03 3.57E-04 -1.24E-02
EP-
kg P eq 1.58E-03 3.07E-06 5.17E-05 3.67E-06 8.8E-08 9.62E-04 0 1.41E-06 6.59E-06 1.25E-05 -3.96E-06
freshwater
EP-marine kg N eq 6.59E-02 3.16E-03 2.81E-03 3.12E-03 2.18E-04 1.77E-01 0 1.31E-03 1.1E-03 8.24E-05 -6.13E-04
EP-terrestrial mol N eq 6.92E-01 3.49E-02 2.84E-02 3.45E-02 2.72E-03 1.86E+00 0 1.45E-02 1.24E-02 9.04E-04 -6.22E-03
kg NMVOC
POCP 2.04E-01 7.48E-03 8.27E-03 5.94E-03 5.7E-04 4.84E-01 0 2.49E-03 2.99E-03 2.65E-04 -2.09E-03
eq
ADPE kg Sb eq 5.57E-03 8.45E-08 5.94E-05 1.22E-06 6.41E-09 1.04E-04 0 3.74E-08 4.93E-07 7.77E-09 -6.17E-04
ADPF MJ 1.25E+03 1.52E+01 4.99E+01 1.51E+01 7.23E-01 6.33E+03 0 6.16E+00 3.06E+01 1.65E+00 -1.72E+01
m3 world eq
WDP 2.54E+01 9.99E-03 1.03E-01 1.67E-02 2.57E-01 7.85E+01 0 4.5E-03 7.93E-01 -1.27E-03 -3.63E-01
deprived
GWP = Global warming potential; ODP = Depletion potential of the stratospheric ozone layer; AP = Acidification potential of land and water; EP =
Eutrophication potential; POCP = Formation potential of tropospheric ozone photochemical oxidants; ADPE = Abiotic depletion potential for non-fossil
resources; ADPF = Abiotic depletion potential for fossil resources; WDP = Water (user) deprivation potential)
RESULTS OF THE LCA - INDICATORS TO DESCRIBE RESOURCE USE according to EN 15804+A2: 1PCS of MAGNA3 40-
120/150/180 (Cast Iron)
Parameter Unit A1 A2 A3 A4 A5 B6 C1 C2 C3 C4 D
PERE MJ 3.27E+02 7.75E-01 3.9E+01 9.47E-01 1.25E-01 2.81E+03 0 3.56E-01 1.32E+01 1.16E-01 6.16E+00
PERM MJ 0 0 0 0 0 0 0 0 0 0 0
PERT MJ 3.27E+02 7.75E-01 3.9E+01 9.47E-01 1.25E-01 2.81E+03 0 3.56E-01 1.32E+01 1.16E-01 6.16E+00
PENRE MJ 1.25E+03 1.25E+03 4.99E+01 1.52E+01 7.23E-01 6.33E+03 0 6.19E+00 3.06E+01 1.65E+00 -1.7E+01
10 Environmental Product Declaration - Grundfos Holding A/S - MAGNA3 40-120/150/180 (Cast Iron)
PENRM MJ 0 0 0 0 0 0 0 0 0 0 0
PENRT MJ 1.25E+03 1.52E+01 4.99E+01 1.52E+01 7.23E-01 6.33E+03 0 6.19E+00 3.06E+01 1.65E+00 -1.7E+01
SM kg 1.32E+01 0 2.31E-01 2.68E-03 0 0 0 0 0 0 0
RSF MJ 1.46E-23 0 0 2.91E-27 0 0 0 0 0 0 0
NRSF MJ 1.71E-22 0 0 3.42E-26 0 0 0 0 0 0 0
FW m3 7.64E-01 9.07E-04 1.92E-02 1.18E-03 6.06E-03 3.25E+00 0 4.15E-04 2.51E-02 2.1E-05 2.65E-02
PERE = Use of renewable primary energy excluding renewable primary energy resources used as raw materials; PERM = Use of renewable primary
energy resources used as raw materials; PERT = Total use of renewable primary energy resources; PENRE = Use of non-renewable primary energy
excluding non-renewable primary energy resources used as raw materials; PENRM = Use of non-renewable primary energy resources used as raw
materials; PENRT = Total use of non-renewable primary energy resources; SM = Use of secondary material; RSF = Use of renewable secondary fuels;
NRSF = Use of non-renewable secondary fuels; FW = Use of net fresh water
RESULTS OF THE LCA – WASTE CATEGORIES AND OUTPUT FLOWS according to EN 15804+A2:
1PCS of MAGNA3 40-120/150/180 (Cast Iron)
Parameter Unit A1 A2 A3 A4 A5 B6 C1 C2 C3 C4 D
HWD kg 2.16E-04 6.17E-07 1.22E-04 7.44E-07 3.75E-09 2.62E-06 0 2.86E-07 1.59E-08 6.61E-09 -3.3E-04
NHWD kg 3.97E+00 2.31E-03 2.75E-01 3.35E-03 7.04E-02 4.49E+00 0 9.81E-04 5.41E-01 1.89E+00 1.45E+00
RWD kg 5.09E-02 2.67E-05 1.38E-03 4.15E-05 3.47E-05 9.61E-01 0 1.14E-05 4.51E-03 1.97E-05 -1.15E-03
CRU kg 0 0 0 0 0 0 0 0 0 0 0
MFR kg 0 0 0 0 0 0 0 0 1.23E+01 0 0
MER kg 0 0 0 0 0 0 0 0 0 0 0
EEE MJ 0 0 0 0 3.21E+00 0 0 0 6.93E+00 0 0
EET MJ 0 0 0 0 5.82E+00 0 0 0 1.25E+01 0 0
HWD = Hazardous waste disposed; NHWD = Non-hazardous waste disposed; RWD = Radioactive waste disposed; CRU = Components for re-use;
MFR = Materials for recycling; MER = Materials for energy recovery; EEE = Exported electrical energy; EET = Exported thermal energy
RESULTS OF THE LCA – additional impact categories according to EN 15804+A2-optional:
1PCS of MAGNA3 40-120/150/180 (Cast Iron)
Parameter Unit A1 A2 A3 A4 A5 B6 C1 C2 C3 C4 D
Disease
PM 6.35E-06 1.2E-07 2.23E-07 3.9E-08 3.41E-09 6.67E-06 0 1.59E-08 3.77E-08 3.64E-09 -2.99E-07
incidence
IR kBq U235 eq 5.61E+00 3.93E-03 2.17E-01 5.78E-03 5.33E-03 1.58E+02 0 1.68E-03 7.4E-01 2.8E-03 -5.89E-02
ETP-fw CTUe 7.8E+02 1.13E+01 1.68E+01 1.11E+01 3.67E-01 2.71E+03 0 4.61E+00 1.34E+01 1.16E+00 -5.83E+00
HTP-c CTUh 1.63E-06 2.31E-10 6.46E-07 6.85E-10 1.8E-11 7.48E-08 0 9.55E-11 4.13E-10 6.66E-11 -6.95E-08
HTP-nc CTUh 2.34E-06 1.25E-08 5.15E-08 1.35E-08 8.68E-10 2.76E-06 0 5.47E-09 1.68E-08 5.81E-09 -4.89E-09
SQP SQP 3.49E+02 4.67E+00 7.08E+01 5.22E+00 1.96E-01 2.02E+03 0 2.16E+00 9.64E+00 1.19E-01 -1.43E+01
PM = Potential incidence of disease due to PM emissions; IR = Potential Human exposure efficiency relative to U235; ETP-fw = Potential comparative
Toxic Unit for ecosystems; HTP-c = Potential comparative Toxic Unit for humans (cancerogenic); HTP-nc = Potential comparative Toxic Unit for humans
(not cancerogenic); SQP = Potential soil quality index
Disclaimer
1 – for the indicator 'Potential Human exposure efficiency relative to U235'.
This impact category deals mainly with the eventual impact of low-dose ionizing
radiation on human health of the nuclear fuel cycle. It does not consider
effects due to possible nuclear accidents, occupational exposure or
radioactive waste disposal in underground facilities. Potential ionizing
radiation from the soil, radon and from some construction materials is
also not measured by this indicator.
Disclaimer 2 – for the
indicators 'abiotic depletion potential for non-fossil resources', 'abiotic
depletion potential for fossil resources', 'water (user) deprivation potential,
deprivation-weighted water consumption', 'potential comparative toxic unit for
ecosystems', 'potential comparative toxic unit for humans – cancerogenic',
'Potential comparative toxic unit for humans - not cancerogenic', 'potential
soil quality index'. The results of this environmental impact indicator shall
be used with care as the uncertainties on these results are high as there is
limited experience with the indicator.
Disclaimer 3: JRC
11 Environmental Product Declaration - Grundfos Holding A/S - MAGNA3 40-120/150/180 (Cast Iron)
Technical Reports, Version 2, 2018 Page 6, for the
indicator "EP-freshwater". This indicator has been calculated as 'kg
P eq' as required in the characterization model EUTREND model, Struijs et al.,
2009b, as implemented in ReCiPe; This EPD was created using a software tool.
References
Standards
EN 15804
Radio Equipment
EN 15804:2012+A1 2013, Sustainability of construction works Directive
— Environmental Product Declarations — Core rules for the
product category of construction products.
EN 15804 DIRECTIVE
2014/53/EU OF THE EUROPEAN PARLIAMENT AND OF THE
EN 15804:2012+A2:2019+AC:2021, Sustainability of COUNCIL of 16 April 2014 on
construction works — Environmental Product Declarations — the harmonisation of the laws of the Member States relating to
Core rules for the product category of construction products. the making
available on the market of
ISO 14025
EN ISO 14025:2011, Environmental labels and declarations —
Type III environmental declarations — Principles and radio equipment
procedures.
Further References
Title of the software/database
Title of the software/database. Addition to the title, version.
Place: Publisher, Date of publication [Access on access date].
Electromagnetic
Compatibility (EMC) Directive
IBU 2021
Institut Bauen und Umwelt e.V.: General Instructions for the
EPD programme of Institut Bauen und Umwelt e.V., Version
DIRECTIVE
2.0, Berlin: Institut Bauen und Umwelt e.V., 2021
2014/30/EU OF THE EUROPEAN
www.ibu-epd.com
Standards
PARLIAMENT AND
OF THE COUNCIL of 26 February
2014 on the
harmonistion of the laws of the Member
Machinery
Directive
States relating
to electromagnetic compatibility
DIRECTIVE 2006/42/EC
OF THE EUROPEAN
PARLIAMENT AND
OF THE COUNCIL of 17 May
Ecodesign
Directive
2006 on
machinery
DIRECTIVE
2009/125/EC OF THE EUROPEAN
12 Environmental Product Declaration - Grundfos Holding A/S - MAGNA3 40-120/150/180 (Cast Iron)
PARLIAMENT AND
PARLIAMENT AND OF THE COUNCIL of 8 June 2011
OF THE COUNCIL of 21 October
on the
2009 restriction of the use of certain hazardous
establishing a framework for the setting of
substances in
ecodesign electrical and electronic equipment
requirements for energy-related products
DIRECTIVE
EC 641/2009 2015/863/EU
COMMISSION DIRECTIVE
REGULATION (EC) No 641/2009 of 22 July 2009 implementing 2015/863/EU of 31 March 2015 amending
Directive 2005/32/EC
of the European Parliament and of the Council with regard to
ecodesign
requirements for glandless standalone circulators and Annex II to
glandless circulators integrated Directive 2011/65/EU of the European
in
Parliament and
products of the Council as regards the list of
restricted
substances
EC 622/2012
COMMISSION
REGULATION (EU) No 622/2012 of 11 July 2012 amending ETSI EN 301
Regulation (EC) No 489-1
641/2009 with regard to ecodesign requirements for glandless
standalone
circulators and glandless circulators integrated in products
ETSI EN 301
489-1 V2.2.0, Electromagnetic Compatibility (EMC) standard for
radio equipment
and services; Part 1: Common technical requirements
DIRECTIVE
2011/65/EU
ETSI EN 301
DIRECTIVE 489-17
2011/65/EU OF THE EUROPEAN
ETSI EN 301
13 Environmental Product Declaration - Grundfos Holding A/S - MAGNA3 40-120/150/180 (Cast Iron)
489-17 V3.2.0, Electromagnetic Compatibility (EMC) standard
for radio equipment EN 55014-2
and services; Part 17: Specific conditions for Broadband Data
Transmission
Systems
EN
55014-2:2015, Electromagnetic compatibility –
Requirements
for household appliances, electric tools
and similar
apparatus – Part 2: Immunity – Product
ETSI EN 300 328 family standard
V2.1.1 (CISPR 14-2:2015)
ETSI EN 300 328
V2.1.1, Wideband transmission systems; Data transmission
equipment operating in
the 2,4 GHz ISM band and using wide band modulation
techniques EN 50581:2012
EN 50581:2012,
Technical documentation for the
EN 809
assessment of
electrical and electronic products with
EN 809:1998-10
+ A1:2009, Pumps and pump units for
respect to the
restriction of hazardous substances
liquids -
Common safety requirements
EN 60335-1
EN 55014-1
EN
60335-1:2012/A11:2014/A13:2017, Household
EN
55014-1:2017, Electromagnetic compatibility – Requirements
for household and similar
appliances, electric tools and similar apparatus – Part 1: electrical appliances – Safety – Part 1:General requirements
Emission
14 Environmental Product Declaration - Grundfos Holding A/S - MAGNA3 40-120/150/180 (Cast Iron)
EN 60335-2-51 EN 16297-1
EN EN
60335-2-51:2003-03 + A1:2008 + A2:2012, Household and 16297-1:2012-10, Pumps – Rotodynamic pumps –Glandless
similar electrical circulators – Part 1:
appliances – Safety –Part 2-51: Particular requirements for General requirements and procedures for testing and
stationary calculation of energy
circulation pumps for heating and service water installations efficiency index (EEI)
EN 61000-3-2
EN
61000-3-2:2014/2019, Electromagnetic compatibility (EMC) –
Part 3-2: Limits –
Limits for harmonic current emissions (equipment input current
=16 A per phase)
EN 16297-2
EN 61000-3-3 EN 16297-2:2012-10,
Pumps – Rotodynamic pumps –Glandless circulators – Part 2:
Calculation of
energy efficiency index (EEI) for standalone circulators
EN
61000-3-3:2013-08/ A1:2019, Electromagnetic compatibility
(EMC) – Part 3-3:
Limits – Limitation of voltage changes, voltage fluctuations and
flicker in public
low voltage supply systems, for equipment with
EN 16297-3
rated current
<= 16 A per phase and not subject to conditional connection
EN
16297-3:2012, Pumps – Rotodynamic pumps –Glandless
circulators – Part 3: Energy
efficiency index (EEI) for circulators integrated in products
EN 61000-6-2
EN ISO 14001
61000-6-2:2008/2019, Electromagnetic compatibility (EMC) –
Part 6-2: Generic
standards –Immunity for industrial environments
EN ISO
14001:2015-09, Environmental management systems -
Requirements with guidance
for use
15 Environmental Product Declaration - Grundfos Holding A/S - MAGNA3 40-120/150/180 (Cast Iron)
and liquids with
solids, Version 1.0 (2018)
ISO 14025
DIN EN /ISO
14025:2011-10, Environmental labels and declarations — Type
III environmental
declarations — Principles and procedures
EN 15804
Further
references
EN
15804:2012-04+A1 2013, Sustainability of construction works
— Environmental
Product Declarations — Core rules for the product category of
construction
products
CPR
REGULATION (EU)
No 305/2011 OF THE EUROPEAN PARLIAMENT AND OF
PCR Part A THE COUNCIL of 9 March 2011
laying down harmonised conditions for the marketing of
construction products
and repealing Council Directive 89/106/EEC
Institut Bauen
und Umwelt e.V., Berlin (pub.): Product Category Rules for
Building-Related
Products and Services, Product Category Rules for
Construction Products from
the range of Environmental Product Declarations of Institut
Bauen und Umwelt
(IBU), Part A: Calculation Rules for the Life Cycle Assessment CML 2001
and Requirements
on the Project Report, Version 1.7 (2021)
Impact
assessment characterization factors Institute of Environmental
Sciences, Leiden
University, Netherlands
PCR
Part B
Institut Bauen ECHA candidate
und Umwelt e.V., Berlin (pub.): Product Category Rules for list
Building-Related
Products and Services, Product Category Rules for
Construction Products from
the range of Environmental Product Declarations of Institut Candidate List
Bauen und Umwelt of substances of very high concern (SVHCs) for authorisation,
(IBU), Part B: Requirements on the EPD for Pumps for liquids European
16 Environmental Product Declaration - Grundfos Holding A/S - MAGNA3 40-120/150/180 (Cast Iron)
Chemicals Agency (ECHA), Helsinki, Finland REACH
Regulation (EC)
No 1907/2006 of the European Parliament and of the Council of
18 December 2006
concerning the Registration, Evaluation, Authorisation and
Ecoinvent Restriction of
Chemicals (REACH) (Status: 27.06.2018)
Ecoinvent v3.5
SVR
GaBi ts
Advisory Board
(formerly SVA)
GaBi ts 9.2.1.68
(database schema 8007)
Decision no.
20170712-n
17 Environmental Product Declaration - Grundfos Holding A/S - MAGNA3 40-120/150/180 (Cast Iron)
Publisher
Institut Bauen und Umwelt e.V. +49 (0)30 3087748- 0
Hegelplatz 1 info@ibu-epd.com
10117 Berlin www.ibu-epd.com
Germany
Programme holder
Institut Bauen und Umwelt e.V. +49 (0)30 3087748- 0
Hegelplatz 1 info@ibu-epd.com
10117 Berlin www.ibu-epd.com
Germany
Author of the Life Cycle Assessment
Grundfos Holding A/S +45 87501400
Poul Due Jensens Vej 7 atomic@grundfos.com
8850 Bjerringbro www.grundfos.com
Denmark
Owner of the Declaration
Grundfos Holding A/S +45 87501400
Poul Due Jensens Vej 7 atomic@grundfos.com
8850 Bjerringbro www.grundfos.com
Denmark
18 Environmental Product Declaration - Grundfos Holding A/S - MAGNA3 40-120/150/180 (Cast Iron)
