ENVIRONMENTAL-PRODUCT DECLARATION
as per ISO 14025 and EN 15804+A2
Owner of the Declaration Grundfos Holding A/S
Publisher Institut Bauen und Umwelt e.V. (IBU)
Programme holder Institut Bauen und Umwelt e.V. (IBU)
Declaration number EPD-GRU-20230069-CBC2-EN
Issue date 31.08.2023
Valid to 30.08.2028
MAGNA3 65-150 (Cast Iron)
Grundfos Holding A/S
www.ibu-epd.com | https://epd-online.com
General Information
Grundfos Holding A/S MAGNA3 65-150 (Cast Iron)
Programme holder Owner of the declaration
IBU – Institut Bauen und Umwelt e.V. Grundfos Holding A/S
Hegelplatz 1 Poul Due Jensens Vej 7
10117 Berlin 8850 Bjerringbro
Germany Denmark
Declaration number Declared product / declared unit
EPD-GRU-20230069-CBC2-EN Name of declared product / declared unit
This declaration is based on the product category rules: Scope:
Pumps for liquids and liquids with solids, 01.08.2021 The declaration applies to 1 piece of MAGNA3 (Cast Iron) pump.
(PCR checked and approved by the SVR)
The product is produced in Wahlstedt, Germany, and the life cycle
assessment is based on data collected at the production site.
Issue date
Production has been modeled using annual production data from 2021.
31.08.2023
The declaration covers MAGNA3 65-150 product.
The owner of the declaration shall be liable for the underlying information
Valid to
and evidence; the IBU shall not be liable with respect to manufacturer
30.08.2028 information, life cycle assessment data and evidences.
The EPD was created according to the specifications of EN 15804+A2. In
the following, the standard will be simplified as EN 15804 bezeichnet.
Verification
The standard EN 15804 serves as the core PCR
Independent verification of the declaration and data according to ISO
14025:2011
internally X externally
Dipl.-Ing Hans Peters
(chairman of Institut Bauen und Umwelt e.V.)
Florian Pronold Mrs Kim Allbury,
(Managing Director Institut Bauen und Umwelt e.V.) (Independent verifier)
1 Environmental-Product Declaration - Grundfos Holding A/S - MAGNA3 65-150 (Cast Iron)
Product
Product description/Product definition
The Grundfos MAGNA3 circulator pumps are designed for
circulating liquids in heating systems, air conditioning and The CE marking takes into account the proof of conformity with
cooling systems and domestic hot water systems. However, the the respective harmonized norms based on the legal provisions
pump range can also be used in ground source heat pump above.
systems and solar heating systems.
MAGNA3 pumps are not harmonized in accordance with the
CPR.
The MAGNA3 pump is a centrifugal pump powered by an
electrical motor. It has a high-performance neodymium magnet Application
rotor which increases motor efficiency and an insulation shell to For the application and use the respective national provisions
reduce heat loss from the cast iron pump housing with threaded apply.
connections.
The pump is designed for circulating liquids in the
The declaration covers MAGNA3 65-150 pump. For the placing
on the market in the European Union/European Free Trade following systems:
Association (EU/EFTA) (with the exception of Switzerland) the
following legal provisions apply: · heating systems
Machinery Directive (2006/42/EC) · domestic hot-water systems
Standard used: EN 809:1998 + A1:2009. · air-conditioning and cooling systems
· ground-source heat-pump systems
Radio Equipment Directive (2014/53/EU) · solar-heating systems
Standards used: The pump is suitable for thin, clean, non-aggressive and non-
EN 60335-1:2012/AC:2014 + A11:2014, EN 60335-2-51:2003 + explosive liquids, not containing solid particles or fibres that
A1:2008 + A2:2012, EN 62233:2008. may attack the pump mechanically or chemically. In heating
systems, the water must meet the requirements of accepted
EN 55014-1:2006 + A1:2009 + A2:2011, EN 55014-1:2017, EN standards on water quality in heating systems. The pumps are
61000-6-2:2005, EN 61000-3-2:2014, EN 61000-3-3:2013, also suitable for domestic hot-water systems.
ETSI EN 301 489-1 V2.2.0, ETSI EN 301 489-17 V3.2.0. ETSI
EN 300 328 V2.1.1 Technical Data
The performance data of the product according to the
harmonized norms, based on the harmonization provisions
above apply.
Electromagnetic Compatibility (EMC) Directive
(2014/30/EU) The relevant technical specifications according to the PCR Part
B are given in the table below.
Standards used: EN 55014-1:2017, EN 55014-2:2015,
EN 61000-3-2:2014/2019, EN 61000-6-2:2008/2019, Note:
Electrical pumps usually falls under the scope of several
EN 61000-3-3:2013 A1:2019 internal market
directives and regulations, such as the Machinery directive,
Ecodesign
Directive, Radio Equipment Directive etc. The relevant technical
RoHS Directive 2011/65/EU and 2015/863//EU data given in
the EPD will vary depending on the type of product and areas
Standard: EN 50581:2012. of application,
and the table below should be adjusted accordingly.
Constructional data
Ecodesign Directive (2009/125/EC)
Commission Regulation (EC) No: 641/2009 and
Commission Regulation (EU) 622/2012
Standards used:
EN 16297-1:2012, EN 16297-2:2012, EN 16297-3:2012.
2 Environmental-Product Declaration - Grundfos Holding A/S - MAGNA3 65-150 (Cast Iron)
Name Value Unit
10.06.2022) exceeding 0.1 percentage by mass: no
Frequency 50 Hz
Voltage 230 V
Energy Efficiency Index 0,17
Flow range 42,5 m3/h The Wahlstedt production has been assessed and certified as
Head max 15 m meeting the requirements in ISO 14001, ISO 50001, ISO 45001
Power input 0,562 kW and ISO 9001.
Nominal capacity 1,271 kW Environment and health during use
The performance data of the product according to the
Reference service life
harmonised norms, based on the harmonisation provisions
above apply. No use stage scenario which refers to the lifetime of the product
is declared. However, to facilitate building calculations, an
Base materials/Ancillary materials estimated RSL of 10 years can be used.
Name Value Unit This is an EU consensus-based estimation, referenced on page
37 in Appendix 7: Lot 11 – Circulators in Buildings, prepared by
Aluminium 15 %
AEA Energy & Environment for the European Commission in
Cast iron 48 %
the context of the Eco Design Directive:
Ceramics 0,3 %
Copper 5 % There is no definitive information on the average circulator life
Electronics 0,2 % available, there is consensus within the industry that it is at
least 12 years. However, this is complicated by many factors,
Magnet Nd 1 %
including many being scrapped prematurely when e.g. the
Paper 0,4 %
boiler they are connected to is replaced.
PCB 3 %
Plastics 0,3 %
Plastics, foam 1 %
Plastics GF 5 % From the estimated stock (140Mpa) and annual sales (14Mpa),
the average lifetime of the circulator is taken as 10 years for the
Rubber 0,1 %
purposes of this study.
Stainless steel 4 %
Steel 11 %
Cardboard 7 %
Plastic film 0,1 % The RSL of the declared product is not directly influencing the
results in this study, as no declared use stage scenario is
TOTAL 100 %
dependent on the RSL; The use stage sub-module B6 is
REACH declared per year as required by the PCR Part B.
This product/article/at least one partial article contains
substances listed in the ECHA candidate list (date:
LCA: Calculation rules
decision no. 20170712-n of the SVR, the modules B3, B4 and
Declared Unit B5 are by default declared as "MNR" (module not relevant).
The declared unit is 1 piece (pcs.) of MAGNA3 (Cast Iron)
pump. The product stage (A1-A3) comprises raw material extraction
Declared unit and processing, transport processes as well as the
manufacturing process. The final production and assembly of
Name Value Unit
the MAGNA3 pump takes place at a Grundfos manufacturing
Declared unit 1 pce.
site in Germany. However, the full supply-chain leading to the
Mass reference 26.3 kg/pce finished product at the gate is rather complex and includes a
Conversion factor [Mass/Declared Unit] 26,3 large amount of raw materials, components and semi-finished
parts which come from both external suppliers as well as other
For IBU core EPDs (where clause 3.6 is part of the EPD): for
Grundfos production facilities.
average EPDs, an estimate of the robustness of the LCA
values must be made, e.g. concerning variability of the
production process, geographical representativeness and the
influence of background data and preliminary products
compared to the environmental impacts caused by actual
production.
The product stage is included in the study, and according to EN
15804 the system boundary with nature is set to include those
System boundary processes that provide the material and energy inputs into the
system and the following manufacturing, transport up to the
This EPD is Cradle-To-Grave. The system boundaries
factory gate as well as the processing any waste arising from
those processes.
of the EPD follow the modular approach in EN 15804. By
3 Environmental-Product Declaration - Grundfos Holding A/S - MAGNA3 65-150 (Cast Iron)
· Transportation from distribution centre to construction site;
Wastes and losses are included in the modules where they
occur according to the polluter pays principle and the modular · Wastage during distribution.
approach of EN 15804.
A5:
· Installation process;
The product includes:
· Transport of packaging waste to treatment site;
· A1 Extraction and processing of raw materials;
· Waste treatment of packaging.
· A1 Reuse of products or materials from a previous product
system; The packaging material does not reach the end of waste state
but is incinerated as waste.
· A1 Processing of secondary materials; According to European statistics, the average R1 value of
incineration plants is > 0.6. Therefore, it is assumed
· A1 Generation of electricity, steam and heat from primary
energy resources, also including their extraction, refining and that packaging material is treated thermally in an incineration
transport; plant with R1 > 0.6. The loads from the combustion process of
packaging are declared in module A5 and the resulting energy
· A1 Energy recovery and other recovery processes from benefits in module
secondary fuels;
D, as required by the PCR Part A, 5.5.2.
· A2 Transportation up to the factory gate and internal transport;
· A3 Production of ancillary materials or pre products;
Use stage (B1-B7):
· A3 Manufacturing of products and coproducts;
· A3 Manufacturing of packaging;
The use stage, related to the building fabric includes:
· A1-A3 processing up to the end-of-waste state or disposal of
final residues. · B1, use or application of the installed product;
For secondary material inputs, the system boundary to the · B2, maintenance.
previous system (providing the secondary material) is set where
outputs reach the end-of-waste state. The recycling of The use stage related to the operation of the building
secondary material into new raw materials is included in the
system boundary of this study. Waste includes:
materials from production processes that are recycled without · B6, operational energy use;
any modification of the material's inherent characteristics are
modelled as closed-loop within A1-A3. This is done up to the · B7, operational water use.
input mass flow that was used during production.
In this study, all use stage modules are assessed, though B1,
B2 and B7 are assessed to be zero. By decision no. 20170712-
n of the SVR, the modules B3, B4 and B5 are by default
Waste for incineration arising in the product stage is accounted declared as "MNR" (module
for in the module where the waste is produced. The
environmental loads from the incineration process are declared not relevant).
in the module where it occurs and the electricity and heat which The modules include the provision and transport of all
is produced from the incineration are considered as closed-loop materials, products and related energy and water use, as well
within A1-A3, as described in PCR Part A, 5.5.1. The input of as waste processing up to the end-of-waste state or disposal of
biogenic carbon from the production of packaging material is final residues during the use stage. They also include all
inventoried in A3. As required by PCR Part A, the impacts and
corresponding end-of-life module of the packaging material, A5,
is also declared and the emissions of biogenic carbon are aspects related to the losses during the use stage (i.e.
inventoried. production, transport, and waste processing and disposal of the
lost products and materials).
The construction process stage (A4-A5) includes:
Generally, the geographical coverage of the datasets used
A4: matches the actual processes taking place. Meaning, that when
modelling taking place in Grundfos Bjerringbro, the Danish
· Transportation from factory gate to distribution centre: electricity grid mix is used in the model and thermal energy
from natural gas. These are generally of very high quality with
· Consumption of electricity, thermal energy and water at very good technological, temporal and geographical
distribution centre; representativeness.
4 Environmental-Product Declaration - Grundfos Holding A/S - MAGNA3 65-150 (Cast Iron)
Contributions to operational energy use during the use stage Materials from which energy is recovered in an incineration
(B6) comes from the electricity consumption of the product. The process with an R1-value above 0.60 are in this study included
annual electricity consumption is calculated by multiplying the with the environmental burdens from the incineration process
average power input, which is based on a defined load profile, inventoried in C3, the recovered energy is declared as exported
with the annual running hours. For use stage (B6) European energy in C3
Average electricity grid mix has been used. These values are
declared in the scenarios section. and the energy benefits are declared in D. This procedure is
according to the PCR Part A, 5.5.6. C3 includes the mechanical
separation of the product followed by a series of sorting steps.
Metal fractions are recycled and plastics, cardboard and
The End-of-Life stage (C1-C4) includes all activities from electronics are assumed incinerated with energy recovery. The
when the product reaches the end of its service life and no residual fractions are landfilled and declared in C4.
longer provides any functionality and until all materials and
components are processed for The specific amounts are shown in the scenarios section.
reuse/recycling or disposed of.
Beyond system boundary (D): According to EN 15804
module D includes the reuse, recovery and/or recycling
According to EN 15804 and the PCR Part A, the end-of-life potentials, expressed as net impacts and benefits. Any
stage includes: declared benefits and loads from net
· C1 deconstruction of the product from the flows leaving the product system that have not been allocated
as co-products and that have passed the end-of-waste state
· building, including initial on-site sorting of the are included in module D.
· materials;
· C2 transportation of the discarded product to a recycling site Contributions to module D comes from waste incineration
and transportation of waste to final disposal; processes in A5 and C3 as well as material recycling in C3. The
specific fractions and net flows are shown in the scenarios
· C3 waste processing, collection of waste fractions from the section.
deconstruction and waste processing of material flows intended
for reuse, recycling and energy recovery; Geographic Representativeness
Land or region, in which the declared product system is
· C4 waste disposal including physical pretreatment and manufactured, used or handled at the end of the product´s
management of the disposal site. lifespan: Germany
At the end of life, the MAGNA3 pump is manually disassembled
Comparability
from the piping system in which it has been installed. The
Basically, a comparison or an evaluation of EPD data is only
definition of the applied end-of-life scenario in this EPD follows
possible if all the data sets to be compared were created
the requirements in the
according to EN 15804 and the building context, respectively
the product-specific characteristics of performance, are taken
PCR Part A, 6.2 regarding complex products, with a
into account. Software and databases used: GaBi ts 9.2.1.68
combination of recycling, thermal waste treatment and
(database schema 8007) Ecoinvent v3.5..
landfilling. 100 % of the material is considered in the end of life
scenario as required by the PCR. An overall collection rate of
90 % has been assumed.
LCA: Scenarios and additional technical information
Characteristic product properties Name ValueUnit
Information on biogenic carbon
Biogenic carbon content in accompanying kg
0.74
packaging C
The biogenic carbon content quantifies the amount of biogenic
carbon in a construction product leaving the factory gate, and it
will be separately declared for the product and for any The following technical scenario information is required for the
accompanying packaging, as required from the PCR Part A. declared modules and optional for non-declared modules.
The Carbon content of Cardboard and Paper is assumed to Modules for which no information is declared can be deleted;
0.46 kg C. Overall, there is an amount of 9 weight-% Carbon in additional information can also be listed if necessary.
the product leaving the factory gate and has to be considered.
The following technical information is a basis for the declared
Information on describing the biogenic Carbon Content at
modules or can be used for developing specific scenarios in the
factory gate
context of a building assessment if modules are not declared
Note: 1 kg of biogenic carbon is equivalent to 44/12 kg of CO2. (MND).
5 Environmental-Product Declaration - Grundfos Holding A/S - MAGNA3 65-150 (Cast Iron)
A5 is not declared including the disposal of the packaging
End of life (C1-C4)
material on the construction site, the amounts of packaging
Name Value Unit
materials included in the LCA calculations must be declared as
technical scenario information for Module A5. Collected as mixed construction waste 24,3 kg
Transportation distance (C2) 500 km
Aluminium for recycling 3,4 kg
Transport from the gate to the site (A4) Steel for recycling 13,6 kg
Name Value Unit Copper for recycling 1,05 kg
Litres of fuel 0,052 l/100km Stainless steel for recycling 0,89 kg
Transport distance 2003 km Plastics for incineration w/energy 1,39 kg
Capacity utilisation (including empty runs) 85 % Electronics for incineration w/energy 0,81 kg
Gross density of products transported 506 kg/m3 Landfilling 3,15 kg
Wastage during distribution 0,02 %
Reuse, recovery and/or recycling potentials (D), relevant
scenario information
Installation into the building (A5)
Name Value Unit
Name ValueUnit
A5, incineration w/energy recov. (LDPE foil) 4,37 MJ
Packaging waste for incineration (LDPE film) 0,031 kg
A5, incineration w/energy recov.
Packaging waste for incineration 7,91 MJ
1,96 kg (Paper/Cardboard)
(Paper/Cardboard)
C3, steel for recycling (net amounts) -0,54 kg
An estimated RSL of 10 years can be used to facilitate building
C3, stainless steel for recycling (net amounts) 0,52 kg
calculations. This is an EU consensus-based estimation,
referenced in Appendix 7: Lot 11 – Circulators in Buildings, C3, aluminium for recycling (net amounts) -0,469 kg
prepared by AEA Energy & Environment for the European C3, copper for recycling (net amounts) 0,451 kg
Commission in the context of the Eco Design Directive. C3, plastics for incineration, w/ energy recov. 1,39 kg
Reference service life C3, electronics for incineration, w/ energy recov. 0,81 kg
Name Value Unit
Life Span according to the manufacturer 10 a
Operational energy use (B6)
Name Value Unit
Electricity consumption 2810 kWh/a
Average power input, 0,562 kW
Running hours (all groups) 5.000 h/a
6 Environmental-Product Declaration - Grundfos Holding A/S - MAGNA3 65-150 (Cast Iron)
LCA: Results
Characterization model: EN 15804 - 2012+A2 - 2019, PEF. By Decision no. 20170712-n of the IBU SVR, the modules B3, B4, B5 are
marked as MNR (module not relevant) as default. The LCA results in module B6 are given on a period of one year, according to PCR
Part B. To obtain the results from module B6 over the entire life cycle, the LCA results of module B6 must be multiplied by the
estimated RSL of 10 years.
DESCRIPTION OF THE SYSTEM BOUNDARY (X = INCLUDED IN LCA; ND = MODULE OR INDICATOR NOT DECLARED; MNR =
MODULE NOT RELEVANT)
BENEFITS
AND LOADS
CONSTRUCTION
BEYOND
PRODUCT STAGE PROCESS USE STAGE END OF LIFE STAGE
THE SYSTEM
STAGE
BOUNDARIE
S
la ire ta m w a Ry lp p u s tro p s n a rT g n iru tc a fu n a M e h t m o rf tro p s n a rTe tis e h t o t e ta g y lb m e s s A e s U e c n a n e tn ia M ria p e R tn e m e c a lp e R tn e m h s ib ru fe R y g re n e la n o ita re p Oe s u re ta w la n o ita re p Oe s u n o itc u rts n o c -e Dn o itilo m e d tro p s n a rT g n is s e c o rp e ts a W la s o p s iD -e s u e R-y re v o c e R-g n ilc y c e Rla itn e to p
A1 A2 A3 A4 A5 B1 B2 B3 B4 B5 B6 B7 C1 C2 C3 C4 D
X X X X X MND MND MNR MNR MNR X MND X X X X X
RESULTS OF THE LCA - ENVIRONMENTAL IMPACT according to EN 15804+A2: 1PCS of MAGNA3 65-150 (Cast Iron)
Parameter Unit A1 A2 A3 A4 A5 B6 C1 C2 C3 C4 D
GWP-total kg CO 2 eq 1.12E+02 1.56E+00 8.53E-01 1.64E+00 2.86E+00 1.14E+03 0 6.77E-01 6.91E+00 1.57E-01 -1.43E+00
GWP-fossil kg CO 2 eq 1.11E+02 1.55E+00 4.1E+00 1.63E+00 1.53E-01 1.13E+03 0 6.72E-01 6.9E+00 1.62E-01 -1.43E+00
GWP-
biogenic kg CO 2 eq 4.56E-01 -2.15E-03 -3.28E+00 -3.26E-03 2.7E+00 3.77E+00 0 -1.13E-03 7.29E-03 -4.87E-03 1.85E-03
GWP-luluc kg CO 2 eq 1.88E-01 1.14E-02 3.67E-02 1.29E-02 9.69E-05 1.64E+00 0 5.47E-03 3.62E-03 1.42E-04 -4.31E-03
kg CFC11
ODP 9.52E-08 2.72E-16 4.07E-09 1.99E-11 5.23E-16 2.49E-11 0 1.24E-16 5.45E-14 3.63E-16 -9.19E-13
eq
AP mol H+ eq 6.08E-01 1.11E-02 1.73E-02 9.49E-03 8.22E-04 2.5E+00 0 3.97E-03 6.2E-03 5.02E-04 -2.52E-02
EP-
kg P eq 1.63E-03 4.31E-06 6.45E-05 5.21E-06 1.2E-07 3.02E-03 0 2.06E-06 9.57E-06 1.76E-05 -5.04E-06
freshwater
EP-marine kg N eq 7.61E-02 3.86E-03 3.33E-03 4.53E-03 3E-04 5.55E-01 0 1.92E-03 1.49E-03 1.16E-04 -1.31E-03
EP-terrestrial mol N eq 8E-01 4.27E-02 3.33E-02 5.02E-02 3.73E-03 5.83E+00 0 2.12E-02 1.65E-02 1.27E-03 -1.36E-02
kg NMVOC
POCP 2.38E-01 8.86E-03 9.55E-03 8.62E-03 7.83E-04 1.52E+00 0 3.64E-03 4.07E-03 3.73E-04 -4.76E-03
eq
ADPE kg Sb eq 7.51E-03 1.17E-07 6.1E-05 1.64E-06 8.71E-09 3.27E-04 0 5.46E-08 7.17E-07 1.09E-08 -1.26E-03
ADPF MJ 1.49E+03 2.06E+01 5.68E+01 2.19E+01 9.85E-01 1.99E+04 0 9.01E+00 4.44E+01 2.32E+00 -2.67E+01
m3 world eq
WDP 2.73E+01 1.39E-02 2.45E-01 2.25E-02 3.52E-01 2.47E+02 0 6.59E-03 9.88E-01 -1.79E-03 -7.85E-01
deprived
GWP = Global warming potential; ODP = Depletion potential of the stratospheric ozone layer; AP = Acidification potential of land and water; EP =
Eutrophication potential; POCP = Formation potential of tropospheric ozone photochemical oxidants; ADPE = Abiotic depletion potential for non-fossil
resources; ADPF = Abiotic depletion potential for fossil resources; WDP = Water (user) deprivation potential)
RESULTS OF THE LCA - INDICATORS TO DESCRIBE RESOURCE USE according to EN 15804+A2: 1PCS of MAGNA3 65-150
(Cast Iron)
Parameter Unit A1 A2 A3 A4 A5 B6 C1 C2 C3 C4 D
PERE MJ 4.05E+02 1.09E+00 5.12E+01 1.36E+00 1.7E-01 8.81E+03 0 5.21E-01 1.93E+01 1.63E-01 7.86E+00
PERM MJ 0 0 0 0 0 0 0 0 0 0 0
PERT MJ 4.05E+02 1.09E+00 5.12E+01 1.36E+00 1.7E-01 8.81E+03 0 5.21E-01 1.93E+01 1.63E-01 7.86E+00
PENRE MJ 1.49E+03 2.06E+01 5.68E+01 2.2E+01 9.86E-01 1.99E+04 0 9.05E+00 4.44E+01 2.32E+00 -2.66E+01
PENRM MJ 0 0 0 0 0 0 0 0 0 0 0
PENRT MJ 1.49E+03 2.06E+01 5.68E+01 2.2E+01 9.86E-01 1.99E+04 0 9.05E+00 4.44E+01 2.32E+00 -2.66E+01
SM kg 1.92E+01 0 2.4E-01 3.89E-03 0 0 0 0 0 0 0
RSF MJ 1.46E-23 0 0 2.91E-27 0 0 0 0 0 0 0
NRSF MJ 1.71E-22 0 0 3.42E-26 0 0 0 0 0 0 0
FW m3 8.42E-01 1.27E-03 2.61E-02 1.66E-03 8.29E-03 1.02E+01 0 6.07E-04 3.27E-02 2.95E-05 2.64E-02
PERE = Use of renewable primary energy excluding renewable primary energy resources used as raw materials; PERM = Use of renewable primary
energy resources used as raw materials; PERT = Total use of renewable primary energy resources; PENRE = Use of non-renewable primary energy
excluding non-renewable primary energy resources used as raw materials; PENRM = Use of non-renewable primary energy resources used as raw
materials; PENRT = Total use of non-renewable primary energy resources; SM = Use of secondary material; RSF = Use of renewable secondary fuels;
NRSF = Use of non-renewable secondary fuels; FW = Use of net fresh water
RESULTS OF THE LCA – WASTE CATEGORIES AND OUTPUT FLOWS according to EN 15804+A2:
1PCS of MAGNA3 65-150 (Cast Iron)
7 Environmental-Product Declaration - Grundfos Holding A/S - MAGNA3 65-150 (Cast Iron)
Parameter Unit A1 A2 A3 A4 A5 B6 C1 C2 C3 C4 D
HWD kg 3.3E-04 8.69E-07 1.22E-04 1.07E-06 5.11E-09 8.23E-06 0 4.18E-07 2.2E-08 9.29E-09 -3.28E-04
NHWD kg 5.17E+00 3.17E-03 2.96E-01 4.73E-03 9.43E-02 1.41E+01 0 1.43E-03 6.9E-01 2.65E+00 2.13E+00
RWD kg 6.25E-02 3.67E-05 1.57E-03 5.79E-05 4.74E-05 3.02E+00 0 1.67E-05 6.58E-03 2.78E-05 -1.06E-03
CRU kg 0 0 0 0 0 0 0 0 0 0 0
MFR kg 0 0 0 0 0 0 0 0 1.9E+01 0 0
MER kg 0 0 0 0 0 0 0 0 0 0 0
EEE MJ 0 0 0 0 4.37E+00 0 0 0 7.44E+00 0 0
EET MJ 0 0 0 0 7.91E+00 0 0 0 1.34E+01 0 0
HWD = Hazardous waste disposed; NHWD = Non-hazardous waste disposed; RWD = Radioactive waste disposed; CRU = Components for re-use;
MFR = Materials for recycling; MER = Materials for energy recovery; EEE = Exported electrical energy; EET = Exported thermal energy
RESULTS OF THE LCA – additional impact categories according to EN 15804+A2-optional:
1PCS of MAGNA3 65-150 (Cast Iron)
Parameter Unit A1 A2 A3 A4 A5 B6 C1 C2 C3 C4 D
Disease
PM 7.32E-06 1.29E-07 2.42E-07 5.64E-08 4.65E-09 2.09E-05 0 2.32E-08 5.24E-08 5.11E-09 -4.01E-07
incidence
IR kBq U235 eq 6.86E+00 5.41E-03 2.47E-01 8.14E-03 7.3E-03 4.95E+02 0 2.46E-03 1.08E+00 3.94E-03 -2.76E-02
ETP-fw CTUe 8.72E+02 1.53E+01 1.84E+01 1.61E+01 4.97E-01 8.51E+03 0 6.74E+00 1.93E+01 1.63E+00 -1.29E+01
HTP-c CTUh 1.65E-06 3.14E-10 6.65E-07 7.98E-10 2.44E-11 2.35E-07 0 1.4E-10 5.8E-10 9.36E-11 -7.02E-08
HTP-nc CTUh 2.66E-06 1.71E-08 5.75E-08 1.95E-08 1.15E-09 8.66E-06 0 8E-09 2.32E-08 8.16E-09 -1.74E-08
SQP SQP 4.39E+02 6.57E+00 9.72E+01 7.59E+00 2.68E-01 6.33E+03 0 3.16E+00 1.4E+01 1.67E-01 -2.33E+01
PM = Potential incidence of disease due to PM emissions; IR = Potential Human exposure efficiency relative to U235; ETP-fw = Potential comparative
Toxic Unit for ecosystems; HTP-c = Potential comparative Toxic Unit for humans (cancerogenic); HTP-nc = Potential comparative Toxic Unit for humans
(not cancerogenic); SQP = Potential soil quality index
Disclaimer 1 – for the indicator 'Potential Human exposure efficiency relative to U235'.
This impact category deals mainly with the eventual impact of low-dose ionizing radiation on human health of the nuclear fuel cycle. It
does not consider effects due to possible nuclear accidents, occupational exposure or radioactive waste disposal in underground
facilities. Potential ionizing radiation from the soil, radon and from some construction materials is also not measured by this indicator.
Disclaimer 2 – for the indicators 'abiotic depletion potential for non-fossil resources', 'abiotic depletion potential for fossil resources',
'water (user) deprivation potential, deprivation-weighted water consumption', 'potential comparative toxic unit for ecosystems', 'potential
comparative toxic unit for humans – cancerogenic', 'Potential comparative toxic unit for humans - not cancerogenic', 'potential soil
quality index'. The results of this environmental impact indicator shall be used with care as the uncertainties on these results are high
as there is limited experience with the indicator.
Disclaimer 3: JRC Technical Reports, Version 2, 2018 Page 6, for the indicator "EP-freshwater". This indicator has been calculated as
'kg P eq' as required in the characterization model EUTREND model, Struijs et al., 2009b, as implemented in ReCiPe;
References
Standards Title of the software/database. Addition to the title, version.
Place: Publisher, Date of publication [Access on access date].
EN 15804
IBU 2021
EN 15804:2012+A1 2013, Sustainability of construction works
— Environmental Product Declarations — Core rules for the Institut Bauen und Umwelt e.V.: General Instructions for the
product category of construction products. EPD programme of Institut Bauen und Umwelt e.V., Version
2.0, Berlin: Institut Bauen und Umwelt e.V., 2021
EN 15804 www.ibu-epd.com
EN 15804:2012+A2:2019+AC:2021, Sustainability of Standards
construction works — Environmental Product Declarations —
Core rules for the product category of construction products.
ISO 14025 Machinery Directive
EN ISO 14025:2011, Environmental labels and declarations — DIRECTIVE 2006/42/EC OF THE EUROPEAN
Type III environmental declarations — Principles and
procedures. PARLIAMENT AND OF THE COUNCIL of 17 May
Further References 2006 on machinery
Title of the software/database
Radio Equipment Directive
8 Environmental-Product Declaration - Grundfos Holding A/S - MAGNA3 65-150 (Cast Iron)
DIRECTIVE 2014/53/EU OF THE EUROPEAN PARLIAMENT Annex II to Directive 2011/65/EU of the European
AND OF THE COUNCIL of 16 April 2014 on the harmonization
of the laws of the Member States relating to the making Parliament and of the Council as regards the list of
available on the market of
restricted substances
radio equipment
ETSI EN 301 489-1
Electromagnetic Compatibility (EMC) Directive
ETSI EN 301 489-1 V2.2.0, Electromagnetic Compatibility
DIRECTIVE 2014/30/EU OF THE EUROPEAN (EMC) standard for radio equipment and services; Part 1:
Common technical requirements
PARLIAMENT AND OF THE COUNCIL of 26 February
2014 on the harmonistion of the laws of the Member
ETSI EN 301 489-17
States relating to electromagnetic compatibility
ETSI EN 301 489-17 V3.2.0, Electromagnetic Compatibility
(EMC) standard for radio equipment and services; Part 17:
Specific conditions for Broadband Data Transmission Systems
Ecodesign Directive
DIRECTIVE 2009/125/EC OF THE EUROPEAN
PARLIAMENT AND OF THE COUNCIL of 21 October
2009 establishing a framework for the setting of
ETSI EN 300 328 V2.1.1
eco-design requirements for energy-related products
ETSI EN 300 328 V2.1.1, Wideband transmission systems;
Data transmission equipment operating in the 2,4 GHz ISM
band and using wide band modulation techniques
EC 641/2009
COMMISSION REGULATION (EC) No 641/2009 of 22 July
2009 implementing Directive 2005/32/EC of the European EN 809
Parliament and of the Council with regard to eco-design
requirements for glandless standalone circulators and EN 809:1998-10 + A1:2009, Pumps and pump units for
glandless circulators integrated in
liquids - Common safety requirements
products
EN 55014-1
EC 622/2012
EN 55014-1:2017, Electromagnetic compatibility –
COMMISSION REGULATION (EU) No 622/2012 of 11 July Requirements for household appliances, electric tools and
2012 amending Regulation (EC) No 641/2009 with regard to similar apparatus – Part 1: Emission
eco-design requirements for glandless standalone circulators
and glandless circulators integrated in products
EN 55014-2
DIRECTIVE 2011/65/EU EN 55014-2:2015, Electromagnetic compatibility –
DIRECTIVE 2011/65/EU OF THE EUROPEAN Requirements for household appliances, electric tools
PARLIAMENT AND OF THE COUNCIL of 8 June 2011 and similar apparatus – Part 2: Immunity – Product
on the restriction of the use of certain hazardous family standard (CISPR 14-2:2015)
substances in electrical and electronic equipment
EN 50581:2012
DIRECTIVE 2015/863/EU EN 50581:2012, Technical documentation for the
DIRECTIVE 2015/863/EU of 31 March 2015 amending assessment of electrical and electronic products with
9 Environmental-Product Declaration - Grundfos Holding A/S - MAGNA3 65-150 (Cast Iron)
index (EEI) for standalone circulators
respect to the restriction of hazardous substances
EN 16297-3
EN 60335-1
EN 16297-3:2012, Pumps – Rotodynamic pumps –Glandless
EN 60335-1:2012/A11:2014/A13:2017, Household circulators – Part 3: Energy efficiency index (EEI) for circulators
integrated in products
and similar electrical appliances – Safety – Part 1: General
requirements
ISO 14001
EN 60335-2-51 EN ISO 14001:2015-09, Environmental management systems -
Requirements with guidance for use
EN 60335-2-51:2003-03 + A1:2008 + A2:2012, Household and
similar electrical appliances – Safety –Part 2-51: Particular
requirements for stationary circulation pumps for heating and
service water installations ISO 14025
DIN EN /ISO 14025:2011-10, Environmental labels and
declarations — Type III environmental declarations —
EN 61000-3-2 Principles and procedures
EN 61000-3-2:2014/2019, Electromagnetic compatibility (EMC)
– Part 3-2: Limits – Limits for harmonic current emissions
(equipment input current =16 A per phase) EN 15804
EN 15804:2012-04+A1 2013, Sustainability of construction
works — Environmental Product Declarations — Core rules for
EN 61000-3-3 the product category of construction products
EN 61000-3-3:2013-08/ A1:2019, Electromagnetic compatibility
(EMC) – Part 3-3:
Limits – Limitation of voltage changes, voltage fluctuations and PCR Part A
flicker in public low voltage supply systems, for equipment with
Institut Bauen und Umwelt e.V., Berlin (pub.): Product Category
rated current <= 16 A per phase and not subject to conditional Rules for Building-Related Products and Services, Product
connection Category Rules for Construction Products from the range of
Environmental Product Declarations of Institute Bauen und
Umwelt (IBU), Part A: Calculation Rules for the Life Cycle
Assessment and Requirements on the Project Report, Version
EN 61000-6-2 1.7 (2021)
EN 61000-6-2:2008/2019, Electromagnetic compatibility (EMC)
– Part 6-2: Generic standards –Immunity for industrial
environments PCR Part B
Institut Bauen und Umwelt e.V., Berlin (pub.): Product Category
Rules for Building-Related Products and Services, Product
EN 16297-1 Category Rules for Construction Products from the range of
Environmental Product Declarations of Institute Bauen und
EN 16297-1:2012-10, Pumps – Rotodynamic pumps – Umwelt (IBU), Part B: Requirements on the EPD for Pumps for
Glandless circulators – Part 1: liquids and liquids with solids, Version 1.0 (2018)
General requirements and procedures for testing and
calculation of energy efficiency index (EEI)
Further references
EN 16297-2
EN 16297-2:2012-10, Pumps – Rotodynamic pumps – CPR
Glandless circulators – Part 2: Calculation of energy efficiency
10 Environmental-Product Declaration - Grundfos Holding A/S - MAGNA3 65-150 (Cast Iron)
REGULATION (EU) No 305/2011 OF THE EUROPEAN
PARLIAMENT AND OF THE COUNCIL of 9 March 2011 laying
down harmonized conditions for the marketing of construction
products and repealing Council Directive 89/106/EEC GaBi ts
GaBi ts 9.2.1.68 (database schema 8007)
CML 2001
Impact assessment characterization factors Institute of REACH
Environmental Sciences, Leiden University, Netherlands
Regulation (EC) No 1907/2006 of the European Parliament and
of the Council of 18 December 2006 concerning the
Registration, Evaluation, Authorization and Restriction of
ECHA candidate list Chemicals (REACH) (Status: 27.06.2018)
Candidate List of substances of very high concern (SVHCs) for
authorization, European Chemicals Agency (ECHA), Helsinki,
Finland SVR
Advisory Board (formerly SVA)
Ecoinvent Decision no.
20170712-n
Ecoinvent v3.5
11 Environmental-Product Declaration - Grundfos Holding A/S - MAGNA3 65-150 (Cast Iron)
Publisher
Institut Bauen und Umwelt e.V. +49 (0)30 3087748- 0
Hegelplatz 1 info@ibu-epd.com
10117 Berlin www.ibu-epd.com
Germany
Programme holder
Institut Bauen und Umwelt e.V. +49 (0)30 3087748- 0
Hegelplatz 1 info@ibu-epd.com
10117 Berlin www.ibu-epd.com
Germany
Author of the Life Cycle Assessment
Grundfos Holding A/S +45 87501400
Poul Due Jensens Vej 7 atomic@grundfos.com
8850 Bjerringbro www.grundfos.com
Denmark
Owner of the Declaration
Grundfos Holding A/S +45 87501400
Poul Due Jensens Vej 7 atomic@grundfos.com
8850 Bjerringbro www.grundfos.com
Denmark
12 Environmental-Product Declaration - Grundfos Holding A/S - MAGNA3 65-150 (Cast Iron)
