ENVIRONMENTAL PRODUCT DECLARATION
as per ISO 14025 and EN 15804+A2
Owner of the Declaration Kronospan Luxembourg S.A.
Publisher Institut Bauen und Umwelt e.V. (IBU)
Programme holder Institut Bauen und Umwelt e.V. (IBU)
Declaration number EPD-KRO-20230159-CBA1-EN
Issue date 11.07.2023
Valid to 10.07.2028
Medium Density Fibreboard (MDF)
Kronospan Luxembourg S.A.
www.ibu-epd.com | https://epd-online.com
General Information
Kronospan Luxembourg S.A. Medium Density Fibreboard (MDF)
Programme holder Owner of the declaration
IBU – Institut Bauen und Umwelt e.V. Kronospan Luxembourg S.A.
Hegelplatz 1 Rue GadderScheier 1
10117 Berlin 4984 Soleuvre
Germany Luxembourg
Declaration number Declared product / declared unit
EPD-KRO-20230159-CBA1-EN 1m3 Kronospan MDF panel
This declaration is based on the product category rules: Scope:
Wood-based panels, 01.08.2021 This document applies to Kronospan MDF, which is composed of wood
(PCR checked and approved by the SVR) shavings, mixed with a resin (melamine urea formaldehyde – MUF).
The declared unit weight is 716.7 kg/m3. LCA data were compiled using
foreground data collected based on billing documents and material
Issue date balances for the period between October 2020 and March 2022. The
declaration holder is responsible for the underlying data and its verification.
11.07.2023
The owner of the declaration shall be liable for the underlying information
and evidence; the IBU shall not be liable with respect to manufacturer
information, life cycle assessment data and evidences.
Valid to
10.07.2028 The EPD was created according to the specifications of EN 15804+A2. In
the following, the standard will be simplified as EN 15804.
Verification
The standard EN 15804 serves as the core PCR
Independent verification of the declaration and data according to ISO
14025:2011
internally X externally
Dipl.-Ing. Hans Peters
(Chairman of Institut Bauen und Umwelt e.V.)
Florian Pronold Mr Olivier Muller,
(Managing Director Institut Bauen und Umwelt e.V.) (Independent verifier)
1 Environmental Product Declaration - Kronospan Luxembourg S.A. - Medium Density Fibreboard (MDF)
Product
Performance data of the product in accordance with the
Product description/Product definition declaration of performance with respect to its essential
MDF (Medium Density Fibreboard) is engineered wood characteristics according to EN13986:2004 + A1:2015 Wood-
products that consist of panels made from a combination of based panels for use in construction. Characteristics,
wood fibres and resin. They are applicable particularly in evaluation of conformity and marking.
furniture such as doors, construction such as mouldings and
indoor products. It is especially suitable for further finishing Base materials/Ancillary materials
(routing, milling, lacquering, laminating and foiling) and a good The MDF panels are made of 80 - 90% of vigin wood, 8 - 18%
substitute for solid wood. of melamine urea formaldehyde resin (MUF), and 2% of other
The Kronobuild® product line includes, as well as standard additives.
MDF, boards with specialist application properties – moisture
resistant MR MDF, Light MDF and Ultra Light MDF, Flame This product contains substances listed in the candidate list
Retardant MDF, Deep Router MDF. For the placing on the (date: 28/02/2023) exceeding 0.1 percentage by mass : NO.
market of the product in the European Union/European Free
Trade Association (EU/EFTA) (with the exception of Reference service life
Switzerland) Regulation (EU) No. 305/2011 (CPR) applies. The The service life is assumed to be 50 years, as MDF is a non-
product needs a declaration of performance taking into structural element of a building.
consideration EN 13986:2004 + A1:2015, Wood-based panels
for use in construction - Characteristics, evaluation of Since no use impacts are quantified (the products do not
conformity and marking - and the CE-marking. For the require energy, maintenance or other reparation process during
application and use the respective national provisions apply its use), this lifetime parameter does not influence the results.
Application
Due to their homogeneous structure, MDF boards can be milled
three-dimensionally and then painted, foil wrapped or faced
with a paper decor in a membrane press.
The main applications of MDF include interior design, furniture
components, decorative features, cladding, partitions, areas
that require protection from moisture, skirting boards /
architrave and window boards / sills.
Technical Data
Technical product groups covered in this EPD are MDF Light,
Standard MDF, Moisture Resistant MDF, Deep Router MDF,
Flame Retardant, Ultra Light MDF.
Technical specification accounts for thicknesses of boards
within the range of 5,5 - 38mm.
Constructional data
Name Value Unit
640 -
Gross density kg/m3
800
5.1 -
Grammage kg/m2
30.4
Bending strength (longitudinal) 17 - 23 N/mm2
Bending strength (transverse) 17 - 23 N/mm2
1900 -
E-module (longitudinal) N/mm2
2700
1900 -
E-module (transverse) N/mm2
2700
Material dampness at delivery 4 - 11 %
0.5 -
Tensile strength rectangular N/mm2
0.65
0.12 -
Thermal conductivity W/(mK)
0.16
Water vapour diffusion resistance factor (wet 15.7 -
-
cup µ)* 22.9
Sound absorption coefficient (frequency range
0.2 %
1000-2000 Hz)*
Formaldehyde emissions E1 acc. to EN 717-1
or E1 DE 2020 ChemVerbotsV (E05) or TSCA - μg/m3
Title VI / CARB P2
2 Environmental Product Declaration - Kronospan Luxembourg S.A. - Medium Density Fibreboard (MDF)
LCA: Calculation rules
Declared Unit System boundary
This declaration applies to 1 m3 of Kronospan MDF panel, with Type of EPD: Cradle-to-grave (with options)
a declared unit weight of 716.7 kg/m3. The system boundaries of the EPD follow the modular
construction system as described by EN 15804.
Declared unit and mass reference
Name Value Unit The LCA considers the following modules:
Declared unit 1 m3
Mass reference 716.7 kg/m3 A1-A3: Manufacturing of pre-products, packaging, ancillary
materials, transport to the factory and production, with the
Layer thickness 0.014 m
associated energy supply and waste handling
Foreground data for the production processes (A1-A3) were A4: Transport to the construction site
collected from the Kronospan production site (Sanem, A5: Installation into the building including disposal of packaging
Luxembourg) and are and representative for the period of C1: Deconstruction (screws disposal and electricity from the
October 2020 to March 2022. The manufacturing data are screwdriver)· C2: Transport to disposal sites
specific to the technologies used in the plant and representative C3: Final product waste disposal for reuse, recycling and
of the local geographical context. Market share data specific to energy recovery
each product category from the year 2021 were used to model C4: Waste disposal, namely incineration and landfill
the transport to building site (module A4). D: Potential for reuse, recovery and/or recycling including
benefits for product incineration from module C4
For the further life cycle stages (modules A5 to D), generic
Geographic Representativeness
inventory data are used.
These processes are not specific to Kronospan products and Land or region, in which the declared product system is
reference data or statistics were applied. The inputs of outputs manufactured, used or handled at the end of the product´s
of these processes were mainly based on the COFIDAB report lifespan: Luxembourg
prepared by FCBA (2012) and associated French EPD ('FDES')
published by FCBA. The shares between various disposal
Comparability
routes for packaging waste (module A5) were based on
Basically, a comparison or an evaluation of EPD data is only
European statistics for the year 2019.
possible if all the data sets to be compared were created
according to EN 15804 and the building context, respectively
The ecoinvent database version 3.8 was used to model
the product-specific characteristics of performance, are taken
background data. The average dataset based on European
into account.
data is used to model the glue production (no specific supplier
data used).
LCA: Scenarios and additional technical information
The refence service life does not affect the results since no use
Characteristic product properties of biogenic carbon impacts are quantified.
Information on describing the biogenic Carbon Content at End of life (C1-C4)
factory gate
Name Value Unit
Name ValueUnit
Collected as mixed construction waste 716.7 kg
kg
Biogenic carbon content in product 278.2 Energy recovery 594.9 kg
C
Landfilling 121.8 kg
Biogenic carbon content in accompanying kg
16.5
packaging C Reuse, recovery and/or recycling potentials (D), relevant
scenario information
Name Value Unit
Transport to the building site (A4) Avoided energy from incineration 8322 MJ
Name Value Unit
Transport distance (truck) 370 km
Gross density of products transported 728.6 kg/m3
Installation into the building (A5)
Name Value Unit
Auxiliary (screw) 1.75 kg
Electricity consumption 0.073 kWh
Material loss 57.3 kg
Product loss to incineration 83 %
Product loss to landfill 17 %
Packaging waste 12.9 kg
3 Environmental Product Declaration - Kronospan Luxembourg S.A. - Medium Density Fibreboard (MDF)
LCA: Results
The results displayed below apply to 1 m3 of Kronospan MDF panel, with a declared unit weight of 716.7 kg/m3.
DESCRIPTION OF THE SYSTEM BOUNDARY (X = INCLUDED IN LCA; ND = MODULE OR INDICATOR NOT DECLARED; MNR =
MODULE NOT RELEVANT)
Benefits and
Construction loads beyond
Product stage Use stage End-of-life stage
process stage the system
boundaries
la ire ta m w a Ry lp p u s tro p s n a rT g n iru tc a fu n a M e h t m o rf tro p s n a rTe tis e h t o t e ta g y lb m e s s A e s U e c n a n e tn ia M ria p e R tn e m e c a lp e R tn e m h s ib ru fe R y g re n e la n o ita re p Oe s u re ta w la n o ita re p Oe s u n o itc u rts n o c -e Dn o itilo m e d tro p s n a rT g n is s e c o rp e ts a W la s o p s iD -e s u e R-y re v o c e R-g n ilc y c e Rla itn e to p
A1 A2 A3 A4 A5 B1 B2 B3 B4 B5 B6 B7 C1 C2 C3 C4 D
X X X X X MND MND MNR MNR MNR MND MND X X X X X
RESULTS OF THE LCA - ENVIRONMENTAL IMPACT according to EN 15804+A2: 1 m3 Kronospan MDF panel
Parameter Unit A1-A3 A4 A5 C1 C2 C3 C4 D
GWP-total kg CO 2 eq -7.81E+02 2.67E+01 9.37E+01 2.95E-02 5.96E+00 0 1.04E+03 -2.49E+02
GWP-fossil kg CO 2 eq 3.3E+02 2.67E+01 4.82E+00 2.85E-02 5.96E+00 0 6.47E+00 -2.49E+02
GWP-biogenic kg CO 2 eq -1.11E+03 2.72E-02 8.89E+01 9.18E-04 5.36E-03 0 1.03E+03 -4.62E-02
GWP-luluc kg CO 2 eq 1.23E+00 9.6E-03 3.24E-03 6.73E-05 2.34E-03 0 2.19E-03 -7.79E-03
ODP kg CFC11 eq 3.94E-05 6.38E-06 4.07E-07 1.44E-09 1.38E-06 0 1.01E-06 -3.49E-05
AP mol H+ eq 1.82E+00 1.11E-01 3.52E-02 1.62E-04 2.42E-02 0 1.93E-01 -3.2E-01
EP-freshwater kg P eq 1.55E-02 1.83E-04 1.86E-04 3.04E-06 4.18E-05 0 1.1E-04 -2.27E-04
EP-marine kg N eq 2.79E-01 3.37E-02 1.26E-02 2.07E-05 7.21E-03 0 9.32E-02 -1.16E-01
EP-terrestrial mol N eq 4.34E+00 3.72E-01 1.34E-01 2.38E-04 7.96E-02 0 1.03E+00 -1.28E+00
kg NMVOC
POCP 1.41E+00 1.2E-01 4.2E-02 6.54E-05 2.44E-02 0 2.72E-01 -4.37E-01
eq
ADPE kg Sb eq 3.82E-03 6.12E-05 4.9E-05 2.68E-07 2.07E-05 0 2.32E-05 -1.47E-04
ADPF MJ 5.59E+03 4.16E+02 5.39E+01 6.07E-01 9E+01 0 8.32E+01 -3.48E+03
m3 world eq
WDP 4.29E+02 1.43E+00 1.06E+00 7.09E-03 2.7E-01 0 1.86E+00 -1.42E+00
deprived
GWP = Global warming potential; ODP = Depletion potential of the stratospheric ozone layer; AP = Acidification potential of land and water; EP =
Eutrophication potential; POCP = Formation potential of tropospheric ozone photochemical oxidants; ADPE = Abiotic depletion potential for non-fossil
resources; ADPF = Abiotic depletion potential for fossil resources; WDP = Water (user) deprivation potential)
RESULTS OF THE LCA - INDICATORS TO DESCRIBE RESOURCE USE according to EN 15804+A2: 1 m3 Kronospan MDF
panel
Parameter Unit A1-A3 A4 A5 C1 C2 C3 C4 D
PERE MJ 1.53E+02 5.3E+00 3.96E+00 1.25E-01 1.27E+00 0 8.32E+03 0
PERM MJ 1.67E+04 0 0 0 0 0 -8.32E+03 0
PERT MJ 1.68E+04 5.3E+00 3.96E+00 1.25E-01 1.27E+00 0 0 0
PENRE MJ 6.07E+03 4.42E+02 5.72E+01 6.37E-01 9.56E+01 0 8.95E+01 -3.86E+03
PENRM MJ 0 0 0 0 0 0 0 0
PENRT MJ 6.07E+03 4.42E+02 5.72E+01 6.37E-01 9.56E+01 0 8.95E+01 -3.86E+03
SM kg 0 0 0 0 0 0 0 0
RSF MJ 6.87E+03 0 0 0 0 0 0 8.32E+03
NRSF MJ 0 0 0 0 0 0 0 0
FW m3 1.32E+01 2.07E-01 1.07E-01 1.01E-02 5.56E-02 0 3.67E-01 -1.97E-01
PERE = Use of renewable primary energy excluding renewable primary energy resources used as raw materials; PERM = Use of renewable primary
energy resources used as raw materials; PERT = Total use of renewable primary energy resources; PENRE = Use of non-renewable primary energy
excluding non-renewable primary energy resources used as raw materials; PENRM = Use of non-renewable primary energy resources used as raw
materials; PENRT = Total use of non-renewable primary energy resources; SM = Use of secondary material; RSF = Use of renewable secondary fuels;
NRSF = Use of non-renewable secondary fuels; FW = Use of net fresh water
RESULTS OF THE LCA – WASTE CATEGORIES AND OUTPUT FLOWS according to EN 15804+A2:
1 m3 Kronospan MDF panel
Parameter Unit A1-A3 A4 A5 C1 C2 C3 C4 D
HWD kg 8.34E-03 1.01E-03 2.56E-04 4.62E-07 2.35E-04 0 1.94E-04 -4.66E-03
NHWD kg 5.33E+01 3.89E+01 1.69E+01 2.12E-03 4.63E+00 0 1.26E+02 -1.9E+00
RWD kg 1.01E-02 2.82E-03 1.72E-04 4.46E-06 6.09E-04 0 3.07E-04 -3.95E-04
CRU kg 0 0 0 0 0 0 0 0
MFR kg 0 0 0 0 0 0 0 0
MER kg 0 0 5.73E+01 0 0 0 5.95E+02 0
EEE MJ 0 0 0 0 0 0 0 0
EET MJ 0 0 9.67E+02 0 0 0 8.32E+03 0
4 Environmental Product Declaration - Kronospan Luxembourg S.A. - Medium Density Fibreboard (MDF)
HWD = Hazardous waste disposed; NHWD = Non-hazardous waste disposed; RWD = Radioactive waste disposed; CRU = Components for re-use;
MFR = Materials for recycling; MER = Materials for energy recovery; EEE = Exported electrical energy; EET = Exported thermal energy
RESULTS OF THE LCA – additional impact categories according to EN 15804+A2-optional:
1 m3 Kronospan MDF panel
Parameter Unit A1-A3 A4 A5 C1 C2 C3 C4 D
Disease
PM 6.82E-05 3.14E-06 4.96E-07 4.48E-10 5.12E-07 0 1.68E-06 -9.97E-07
incidence
IR kBq U235 eq 7.63E+00 1.81E+00 1.44E-01 5.45E-03 3.91E-01 0 2.43E-01 -3.26E-01
ETP-fw CTUe 7.12E+03 3.25E+02 1.34E+02 3.84E-01 7.03E+01 0 1.49E+02 -2.8E+02
HTP-c CTUh 5.27E-07 8.99E-09 4.4E-08 1.18E-11 2.28E-09 0 1.78E-07 -1.5E-08
HTP-nc CTUh 7.65E-06 3.56E-07 1.76E-07 3.77E-10 7.37E-08 0 5.41E-07 -7.85E-07
SQP SQP 3.36E+04 4.76E+02 2.89E+01 1.1E-01 6.19E+01 0 8.79E+01 -6.8E+01
PM = Potential incidence of disease due to PM emissions; IR = Potential Human exposure efficiency relative to U235; ETP-fw = Potential comparative
Toxic Unit for ecosystems; HTP-c = Potential comparative Toxic Unit for humans (cancerogenic); HTP-nc = Potential comparative Toxic Unit for humans
(not cancerogenic); SQP = Potential soil quality index
Disclaimer 1 – for the indicator “Potential Human exposure efficiency relative to U235”. This impact category deals mainly with the
eventual impact of low-dose ionizing radiation on human health of the nuclear fuel cycle. It does not consider effects due to possible
nuclear accidents, occupational exposure or radioactive waste disposal in underground facilities. Potential ionizing radiation from the
soil, radon and from some construction materials is also not measured by this indicator.
Disclaimer 2 – for the indicators “abiotic depletion potential for non-fossil resources”, “abiotic depletion potential for fossil resources”,
“water (user) deprivation potential, deprivation-weighted water consumption”, “potential comparative toxic unit for ecosystems”,
“potential comparative toxic unit for humans – cancerogenic”, “Potential comparative toxic unit for humans - not cancerogenic”,
“potential soil quality index”. The results of this environmental impact indicator shall be used with care as the uncertainties on these
results are high as there is limited experience with the indicator.
References
Standards produits bois. Convention DHUP/CSTB 2009 Action 33 – Sous
action 5. ACV & Déclarations environnementales pour des
EN 15804 produits et composants de la construction bois.
EN 15804:2012+A2:2019+AC:2021, Sustainability of
construction works — Environmental Product Declarations — FCBA (2019)
Core rules for the product category of construction products. Fiche de déclaration environmentale et sanitaire (FDES) –
Panneaux de lamelles de bois minces orientées OSB (oriented
ISO 14025 strand board) de type 3 (panneaux travaillants utilisés en milieu
EN ISO 14025:2011, Environmental labels and declarations — humide) bruts. Epaisseur déclarée : 18 mm. FDES collective 2-
Type III environmental declarations — Principles and 90 :2018.
procedures.
FCBA (2022a)
EN 13986 Fiche de déclaration environmentale et sanitaire (FDES) –
EN 13986:2004 + A1:2015 Wood-based panels for use in Panneaux de lamelles de bois minces orientées OSB (oriented
construction - Characteristics, evaluation of conformity and strand board) de type 3 (panneaux travaillants utilisés en milieu
marking humide) bruts. Epaisseur déclarée : 12 mm. FDES collective
132289692502022.
Further References
FCBA (2022b)
PCR 2021, Part A Fiche de déclaration environmentale et sanitaire (FDES) –
PCR Guidance-Texts for Building-Related Products and Panneaux de fibres MDF (medium-density fibrebord) utilisés en
Services: Calculation Rules for the Life Cycle Assessment and milieu humide bruts. Epaisseur déclarée : 18 mm.
Requirements on the Project Report according to EN FDES collective 182289782502022.
15804+A2:2019
FCBA (2022c)
PCR 2023, Part B Fiche de déclaration environmentale et sanitaire (FDES) –
PCR-Guidances-Texts for Building-Related Products and Panneaux de fibres MDF (medium-density fibrebord) utilisés en
Services. Part B: Requirements on the EPD for Wood based milieu humide bruts. Epaisseur déclarée : 19 mm. FDES
panels collective 341289752502022.
FCBA (2012) SimaPro software and ecoinvent database:2021
Rapport d'étude Volet 2 – Prise en compte de la fin de vie des SimaPro software ecoinvent database, version 3.8, 2021
5 Environmental Product Declaration - Kronospan Luxembourg S.A. - Medium Density Fibreboard (MDF)
Publisher
Institut Bauen und Umwelt e.V. +49 (0)30 3087748- 0
Hegelplatz 1 info@ibu-epd.com
10117 Berlin www.ibu-epd.com
Germany
Programme holder
Institut Bauen und Umwelt e.V. +49 (0)30 3087748- 0
Hegelplatz 1 info@ibu-epd.com
10117 Berlin www.ibu-epd.com
Germany
Author of the Life Cycle Assessment
Luxembourg Institute of Science and Technology 00352-275888-1
(LIST) info@list.lu
Avenue des Hauts-Fourneaux 5 www.list.lu
4362 Esch/Alzette
Luxembourg
Owner of the Declaration
Kronospan Luxembourg S.A. +352590311214
Rue GadderScheier 1 j.guerlot@kronospan.lu
4984 Soleuvre www.kronospan.lu
Luxembourg
6 Environmental Product Declaration - Kronospan Luxembourg S.A. - Medium Density Fibreboard (MDF)
