ENVIRONMENTAL PRODUCT DECLARATION
as per ISO 14025 and EN 15804+A2
Owner of the Declaration Li&Co AG
Publisher Institut Bauen und Umwelt e.V. (IBU)
Programme holder Institut Bauen und Umwelt e.V. (IBU)
Declaration number EPD-LIC-20230312-CCA1-EN
Issue date 21.12.2023
Valid to 20.12.2028
Micodur - Resilient Floor Covering
Li&Co AG
www.ibu-epd.com | https://epd-online.com
General Information
Li&Co AG Micodur - Resilient Floor Covering
Programme holder Owner of the declaration
IBU – Institut Bauen und Umwelt e.V. Li&Co AG
Hegelplatz 1 Palü Daint 12
10117 Berlin 7537 Müstair
Germany Switzerland
Declaration number Declared product / declared unit
EPD-LIC-20230312-CCA1-EN 1 m² Li&Co Micodur - Resilient Floor Covering
This declaration is based on the product category rules: Scope:
Floor coverings, 01.08.2021 This document relates to the Micodur product manufactured by Li&Co AG
(PCR checked and approved by the SVR) in Müstair (GR), Switzerland.
The owner of the declaration shall be liable for the underlying information
and evidence; the IBU shall not be liable with respect to manufacturer
Issue date information, life cycle assessment data and evidences.
21.12.2023
The EPD was created according to the specifications of EN 15804+A2. In
the following, the standard will be simplified as EN 15804.
Valid to
Verification
20.12.2028
The standard EN 15804 serves as the core PCR
Independent verification of the declaration and data according to ISO
14025:2011
internally X externally
Dipl.-Ing. Hans Peters
(Chairman of Institut Bauen und Umwelt e.V.)
Florian Pronold Ms Jane Anderson,
(Managing Director Institut Bauen und Umwelt e.V.) (Independent verifier)
1 Environmental Product Declaration - Li&Co AG - Micodur - Resilient Floor Covering
Product
at www.lico.ch.
Product description/Product definition
Li&Co Micodur is an elastic, multi-layer and decorative floor
covering in the form of a plank or a tile. The floor has a The floor coverings have a high-performance surface layer and
multilayer structure, which integrates a mineral fiber cement are suitable products for areas with heavy traffic, such as
board (HDF), a lignin sound underlay and an elastic commercial, business, or general public areas. This floating
intermediate layer which is digitally printed with a decor and flooring product meets the requirements of the usage classes
sealed with an abrasion-resistant, UV-curing lacquer 33 for commercial use and 23 for domestic use according to EN
compound. An authentic wood or stone structure can be 16511. Class 33 products are suitable for commercial areas
applied. The edges of the product are processed with a click with high traffic.
connection which enables a form-fitting assembly of the product
to form a larger, flat unit. The product is laid as a floating floor Technical Data
system and is declared according to product standard EN The technical data of the products are tested according to EN
16511. The product corresponds to class 33. 16511. The corresponding data sheets (TDS) for the products
can be sent on request (info@lico.ch).
Technical Data
Name Value Unit
Total thickness 7.5 mm
Grammage 12000 - 13000 g/m²
Abrasion Class 33 -
Reaction of Fire A2fl-s1
Thermal resistance 0,05 m2 K/W
Slip resistance R10
Formaldehyd <60 μg/m³
Pentachlorphenol 0,00 μg/m³
Sustainability: The values correspond to the declaration of performance
Li&Co offers its customers the Second Life service with the aim related to its essential properties according to EN
of sustainably extending the lifespan of Micodur. In this way, 16511:2014+A1:2019, Panels for floating installation - Semi-
Lico makes a decisive contribution to ensuring that floor rigid, multi-layer, modular floor coverings (MMF) with abrasion-
coverings that have already been used are remanufactured. As resistant top layer.
a result, natural resources can be saved and the environmental
impact during the process of remanufacturing can be reduced Base materials/Ancillary materials
to a minimum. One m² of Li&Co Micodur, averaged over the amount that was
www.lico.ch/en/company/innovation-sustainability/second-life/ produced in one year, consists of the following material
components (in mass %)
Name Value Unit
Lignin Sound Underlay 6 %
Regulation (EU) No. 305/2011(CPR) applies to market the
Mineral Core Board 88 %
product in the EU/EFTA (with the exception of Switzerland). The
product requires a declaration of performance according to EN Adhesive 0,4 %
16511:2014+A1:2019, Panels for floating installation - Semi- Elastic Intermediate Layer 2 %
rigid, multi-layer, modular floor coverings (MMF) with abrasion PU-Acrylic Primer and Ink 1,6 %
resistant top layer and the CE marking. The respective national
PUR Lacquer Compound 2 %
regulations apply. A declaration of performance is available and
can be sent on request (info@lico.ch). The product contains substances from the ECHA list of
substances of very high concern (SVHC) (date April 14, 2023)
Application that are eligible for authorization above 0.1% by mass: No.
Li&Co Micodur (either tile or plank form) is a multi-layer, semi-
rigid, modular flooring for commercial and residential use, Reference service life
manufactured in accordance with EN 16511. Depending on the According to the BBSR table "Useful lives of components for
application the floor covering is laid indoors on screed or other life cycle analysis according to "BNB" the useful life is 20 years
subfloors such as wood, tiles or plastic as a floating floor or fully (code no. 352.711). No damage is to be expected if used,
glued. The substrate must be clean, resistant to tension and maintained, cared for and cleaned as recommended. A service
pressure, permanently dry and level. The laying is to be carried life in accordance with the BBSR table is not a RSL (reference
out in accordance with the laying instructions and the state of service life) according to ISO 15686.
the art. The installation instructions are available for download
LCA: Calculation rules
Name Value Unit
Declared Unit
Declared unit 1 m2
1 m² of floor covering.
Layer thickness 0.0075 m
Grammage 12.94 kg/m2
2 Environmental Product Declaration - Li&Co AG - Micodur - Resilient Floor Covering
to waste processing (100km).
System boundary Module C3/1: reuse (second life) of cement fiber board (80-
Type of EPD: cradle to gate with options, modules C1–C4, and 85% of the total product weight) and the rest in landfill
module D (A1–A3, C, D and additional modules: A4, A5 and
B2). Module C4/2: 100% Landfill
Modules A1-A3 include processes that provide materials and Module D/2 Scenario 1: potential benefits given in module A5
energy input for the system, and credit for core material (Cement fiber board) from C3/1 are
manufacturing and transport processes up to the factory gate, declared.
as well as waste processing.
Module A4 includes transport of the floor covering to the place
of installation (100km). Geographic Representativeness
Land or region, in which the declared product system is
Module A5 includes the incineration of packaging material. No manufactured, used or handled at the end of the product´s
adhesives are declared in the EPD. lifespan: Europe
Module B2 is including provision of cleaning agent, energy and
Comparability
water consumption for the cleaning of the floor covering incl.
waste water treatment. The LCA results in this EPD are Basically, a comparison or an evaluation of EPD data is only
declared for a one-year usage. possible if all the data sets to be compared were created
according to EN 15804 and the building context, respectively
Module C1 considers the manual deconstruction. the product-specific characteristics of performance, are taken
into account. The data was collected for the year 2021.
Module C2 includes transportation of the postconsumer waste The used database is LCA FE (GaBi) 2022, version 2022.2.
LCA: Scenarios and additional technical information
The production of the following packaging materials is included
Characteristic product properties of biogenic carbon in the life cycle assessment
Name Value Unit
Information on describing the biogenic carbon content at Carton 0.27 kg
factury gate
Wooden pallet 0.15 kg
Name ValueUnit
kg Maintenance (B2) per year
Biogenic carbon content in product 1.33
C Name Value Unit
Biogenic carbon content in accompanying kg Water consumption 0.003 m3
0.19
packaging C
Auxiliary 0.04 kg
Note: 1 kg of biogenic carbon is equivalent to 44/12 kg of CO . Electricity consumption 0.55 kWh
2
End of life (C1-C4)
Name Value Unit
Transport to the building site (A4) Reuse (Scenario 1) 10.7 kg
Name Value Unit Landfilling (Scenario 2) 12.94 kg
Litres of fuel 0.028 l/100km
Reuse, recovery and/or recycling potentials (D), relevant
Transport distance 100 km scenario information
Capacity utilisation (including empty runs) 61 % For module D/2 the potential benefits given in module A5 and
Vehicle Type Euro 6 credit for core material (Fiber cement board) from C3/1 are
declared.
Einbau ins Gebäude (A5)
Name Value Unit
In A5, only the effort for the thermal recycling of the of the
Core material (Fiber cement board) 10.7 kg
packaging materials are declared. The credits from energy
substitution are declared in D.
3 Environmental Product Declaration - Li&Co AG - Micodur - Resilient Floor Covering
LCA: Results
DESCRIPTION OF THE SYSTEM BOUNDARY (X = INCLUDED IN LCA; MND = MODULE OR INDICATOR NOT DECLARED; MNR
= MODULE NOT RELEVANT)
Benefits and
Construction loads beyond
Product stage Use stage End of life stage
process stage the system
boundaries
la ire ta m w a Ry lp p u s tro p s n a rT g n iru tc a fu n a M e h t m o rf tro p s n a rTe tis e h t o t e ta g y lb m e s s A e s U e c n a n e tn ia M ria p e R tn e m e c a lp e R tn e m h s ib ru fe R y g re n e la n o ita re p Oe s u re ta w la n o ita re p Oe s u n o itc u rts n o c -e Dn o itilo m e d tro p s n a rT g n is s e c o rp e ts a W la s o p s iD -e s u e R-y re v o c e R-g n ilc y c e Rla itn e to p
A1 A2 A3 A4 A5 B1 B2 B3 B4 B5 B6 B7 C1 C2 C3 C4 D
X X X X X MND X MNR MNR MNR MND MND X X X X X
RESULTS OF THE LCA - ENVIRONMENTAL IMPACT according to EN 15804+A2: 1 m² Micodur floor covering (12.94 kg/m²)
Parameter Unit A1-A3 A4 A5 B2 C1 C2 C3/1 C4/2 D/1
GWP-total kg CO 2 eq 9.75E+00 9.18E-02 7.09E-01 2.62E-01 0 8.89E-02 1.02E+01 1.55E+01 -5.25E+00
GWP-fossil kg CO 2 eq 1.51E+01 9.16E-02 1.31E-02 2.61E-01 0 8.88E-02 2.65E+00 1.5E+00 -5.14E+00
GWP-biogenic kg CO 2 eq -5.57E+00 1.5E-04 6.96E-01 7.58E-04 0 1.46E-04 4.87E+00 4.87E+00 -4.68E-04
GWP-luluc kg CO 2 eq 1.91E-01 1.13E-06 2.21E-06 1.68E-05 0 1.09E-06 2.64E+00 3.96E-04 -1.24E-03
ODP kg CFC11 eq 1.44E-10 5.61E-15 6.28E-14 2.27E-12 0 5.43E-15 2.64E+00 9.38E-13 -4.36E-12
AP mol H+ eq 4.82E-02 7.6E-05 1.44E-04 3.84E-04 0 7.37E-05 2.64E+00 3.56E-03 -2.56E-02
EP-freshwater kg P eq 3.01E-04 1.84E-08 1.81E-08 8.34E-07 0 1.79E-08 2.64E+00 2.71E-04 -2.03E-05
EP-marine kg N eq 1.55E-02 2.5E-05 5.1E-05 1.09E-04 0 2.42E-05 2.64E+00 3.07E-03 -5.2E-03
EP-terrestrial mol N eq 1.91E-01 2.78E-04 6.62E-04 1.15E-03 0 2.69E-04 2.64E+00 1.28E-02 -5.66E-02
kg NMVOC
POCP 4.45E-02 7.35E-05 1.36E-04 3.36E-04 0 7.12E-05 2.64E+00 7.34E-03 -1.57E-02
eq
ADPE kg Sb eq 3.88E-06 3.74E-09 1.54E-09 4.51E-08 0 3.62E-09 2.64E+00 4.93E-08 -3.33E-07
ADPF MJ 2.16E+02 1.24E+00 1.72E-01 5.63E+00 0 1.2E+00 5.02E+00 1E+01 -3.66E+01
m3 world eq
WDP 9.79E-01 1.7E-04 7.56E-02 1.11E-01 0 1.65E-04 2.64E+00 4.82E-02 -2.33E-01
deprived
GWP = Global warming potential; ODP = Depletion potential of the stratospheric ozone layer; AP = Acidification potential of land and water; EP =
Eutrophication potential; POCP = Formation potential of tropospheric ozone photochemical oxidants; ADPE = Abiotic depletion potential for non-fossil
resources; ADPF = Abiotic depletion potential for fossil resources; WDP = Water (user) deprivation potential)
RESULTS OF THE LCA - INDICATORS TO DESCRIBE RESOURCE USE according to EN 15804+A2: 1 m² Micodur floor
covering (12.94 kg/m²)
Parameter Unit A1-A3 A4 A5 B2 C1 C2 C3/1 C4/2 D/1
PERE MJ 1.31E+02 4.67E-03 6.89E+00 7.19E-01 0 4.52E-03 4.21E-01 8.22E-01 -3.61E+00
PERM MJ 4.23E+01 0 -6.86E+00 0 0 0 -3.54E+01 0 0
PERT MJ 1.73E+02 4.67E-03 3.94E-02 7.19E-01 0 4.52E-03 -3.5E+01 8.22E-01 -3.61E+00
PENRE MJ 2.06E+02 1.24E+00 1.73E-01 5.65E+00 0 1.2E+00 2.9E+00 1E+01 -4.93E+00
PENRM MJ 1.06E+01 0 0 0 0 0 -1.06E+01 0 0
PENRT MJ 2.17E+02 1.24E+00 1.73E-01 5.65E+00 0 1.2E+00 -7.7E+00 1E+01 -3.66E+01
SM kg 0 0 0 0 0 0 0 0 1.07E+01
RSF MJ 0 0 0 0 0 0 0 0 0
NRSF MJ 0 0 0 0 0 0 0 0 0
FW m3 1.06E-01 7.05E-06 1.78E-03 3.28E-03 0 6.82E-06 1.04E-03 1.42E-03 -6.89E-03
PERE = Use of renewable primary energy excluding renewable primary energy resources used as raw materials; PERM = Use of renewable primary
energy resources used as raw materials; PERT = Total use of renewable primary energy resources; PENRE = Use of non-renewable primary energy
excluding non-renewable primary energy resources used as raw materials; PENRM = Use of non-renewable primary energy resources used as raw
materials; PENRT = Total use of non-renewable primary energy resources; SM = Use of secondary material; RSF = Use of renewable secondary fuels;
NRSF = Use of non-renewable secondary fuels; FW = Use of net fresh water
RESULTS OF THE LCA – WASTE CATEGORIES AND OUTPUT FLOWS according to EN 15804+A2:
1 m² Micodur floor covering (12.94 kg/m²)
Parameter Unit A1-A3 A4 A5 B2 C1 C2 C3/1 C4/2 D/1
HWD kg 9.15E-08 4.09E-12 1.7E-11 3.88E-10 0 3.96E-12 3.46E-10 1.53E-09 -3.12E-09
NHWD kg 2.92E-01 1.16E-04 1.39E-02 2.86E-03 0 1.12E-04 1.77E+00 1.04E+01 -2.42E-01
RWD kg 5.04E-03 1.36E-06 9.62E-06 8.1E-04 0 1.32E-06 8.69E-04 1.22E-04 -5.81E-04
CRU kg 0 0 0 0 0 0 1.07E+01 0 0
MFR kg 0 0 0 0 0 0 0 0 0
MER kg 0 0 0 0 0 0 0 0 0
EEE MJ -1.61E-01 0 -9.72E-01 0 0 0 0 0 0
EET MJ -3.67E-01 0 -1.76E+00 0 0 0 0 0 0
4 Environmental Product Declaration - Li&Co AG - Micodur - Resilient Floor Covering
HWD = Hazardous waste disposed; NHWD = Non-hazardous waste disposed; RWD = Radioactive waste disposed; CRU = Components for re-use;
MFR = Materials for recycling; MER = Materials for energy recovery; EEE = Exported electrical energy; EET = Exported thermal energy
RESULTS OF THE LCA – additional impact categories according to EN 15804+A2-optional:
1 m² Micodur floor covering (12.94 kg/m²)
Parameter Unit A1-A3 A4 A5 B2 C1 C2 C3/1 C4/2 D/1
Disease
PM 1.62E-06 4.07E-10 7.65E-10 3.37E-09 0 3.94E-10 6.28E-09 3.55E-08 -2.99E-07
incidence
IR kBq U235 eq 7.53E-01 1.98E-04 1.56E-03 1.18E-01 0 1.92E-04 9.17E-02 1.8E-02 -7.91E-02
ETP-fw CTUe 1.09E+02 8.61E-01 8.06E-02 1.84E+00 0 8.34E-01 3.7E+00 1.49E+01 -7.08E+00
HTP-c CTUh 4.73E-09 1.59E-11 4.71E-12 3.62E-11 0 1.54E-11 1E-10 5.35E-10 -8.28E-10
HTP-nc CTUh 4.3E-07 6.6E-10 1.9E-10 1.9E-09 0 6.39E-10 9.3E-09 5.19E-08 -7.76E-08
SQP SQP 1.92E+03 3.41E-03 4.93E-02 4.55E-01 0 3.31E-03 5.33E-01 7.81E-01 -3.9E+00
PM = Potential incidence of disease due to PM emissions; IR = Potential Human exposure efficiency relative to U235; ETP-fw = Potential comparative
Toxic Unit for ecosystems; HTP-c = Potential comparative Toxic Unit for humans (cancerogenic); HTP-nc = Potential comparative Toxic Unit for humans
(not cancerogenic); SQP = Potential soil quality index
Disclaimer 1 – for the indicator “Potential Human exposure efficiency relative to U235”. This impact category deals mainly with the
eventual impact of low-dose ionizing radiation on human health of the nuclear fuel cycle. It does not consider effects due to possible
nuclear accidents, occupational exposure or radioactive waste disposal in underground facilities. Potential ionizing radiation from the
soil, radon and from some construction materials is also not measured by this indicator.
Disclaimer 2 – for the indicators “abiotic depletion potential for non-fossil resources”, “abiotic depletion potential for fossil resources”,
“water (user) deprivation potential, deprivation-weighted water consumption”, “potential comparative toxic unit for ecosystems”,
“potential comparative toxic unit for humans – cancerogenic”, “Potential comparative toxic unit for humans - not cancerogenic”,
“potential soil quality index”. The results of this environmental impact indicator shall be used with care as the uncertainties on these
results are high as there is limited experience with the indicator.
References
(EU) No 305/2011 of the European parliament and of the
Standards council of 9 March 2011 laying down harmonised conditions for
EN 16511 the marketing of construction products and repealing Council
EN 16511:2014+A1:2019, Loose-laid panels - Semi-rigid Directive 89/106/EEC
multilayer modular floor covering (MMF) panels with wear
resistant top layer. LCA FE (GaBi) documentation
GaBi life cycle inventory data documentation
(https://www.gabisoftware.com/support/gabi/gabidatabase2020lcidocumentation/)
EN 15804
EN 15804:2012+A1 2013, Sustainability of construction works LCA FE (GaBi) software
— Environmental Product Declarations — Core rules for the Sphera Solutions GmbH, GaBi Software System and Database
product category of construction products. for Life Cycle Engineering, CUP Version: 2022.2, University of
Stuttgart, Leinfelden Echterdingen.
EN 15804 IBU 2021
EN 15804:2012+A2:2019+AC:2021, Sustainability of Institut Bauen und Umwelt e.V.: General Instructions for the
construction works — Environmental Product Declarations — EPD programme of Institut Bauen und Umwelt e.V., Version
Core rules for the product category of construction products. 2.0, Berlin: Institut Bauen und Umwelt e.V., 2021 www.ibu-
epd.com
ISO 14025
EN ISO 14025:2011, Environmental labels and declarations — PCR Part A
Type III environmental declarations — Principles and Institut Bauen und Umwelt e.V., Berlin (pub.): Product Category
procedures. Rules for Construction Products from the range of
Environmental Product Declarations of Institut Bauen und
Further References Umwelt (IBU), Part A: Calculation Rules for the Life Cycle
Assessment and Requirements on the
BNB Background Report. version 1.3, 08/2021 www.bau-umwelt.de
BBSR table (german): 'Nutzungsdauern von
Bauteilen zur Lebenszyklusanalyse nach BNB', Bundesinstitut PCR Part B
für Bau-, Stadt- und Raumforschung, Referat II Nachhaltiges Institut Bauen und Umwelt e.V., Berlin (pub.): Product Category
Bauen; online available under Rules for Construction Products from the range of
https://www.nachhaltigesbauen.de/austausch/nutzungsdauern- Environmental Product Declarations of Institut Bauen und
von-bauteilen/ Umwelt (IBU), Part B: Requirements on the EPD for
floorcoverings, Institut Bauen und Umwelt e.V., www.bau-
CPR Regulation umwelt.com, version 4, 06/2023
5 Environmental Product Declaration - Li&Co AG - Micodur - Resilient Floor Covering
Publisher
Institut Bauen und Umwelt e.V. +49 (0)30 3087748- 0
Hegelplatz 1 info@ibu-epd.com
10117 Berlin www.ibu-epd.com
Germany
Programme holder
Institut Bauen und Umwelt e.V. +49 (0)30 3087748- 0
Hegelplatz 1 info@ibu-epd.com
10117 Berlin www.ibu-epd.com
Germany
Author of the Life Cycle Assessment
Sphera Solutions GmbH +49 711 341817-0
Hauptstraße 111- 113 info@sphera.com
70771 Leinfelden-Echterdingen www.sphera.com
Germany
Owner of the Declaration
Li&Co AG +41 (0)81 850 38 38
Palü Daint 12 info@lico.ch
7537 Müstair www.lico.ch
Switzerland
6 Environmental Product Declaration - Li&Co AG - Micodur - Resilient Floor Covering
