ENVIRONMENTAL PRODUCT DECLARATION
as per ISO 14025 and EN 15804+A2
Owner of the Declaration
Programme holder Institut Bauen und Umwelt e.V. (IBU)
Publisher Institut Bauen und Umwelt e.V. (IBU)
Declaration number EPD­ZIN­20210263­IBG1­EN
Issue date 22.03.2022
Valid to 21.03.2027
microZINQ® hot-dip galvanized steel
ZINQ Technologie GmbH
www.ibu-epd.com | https://epd-online.com
Umwelt Produktdeklaration Name des Herstellers – Name des Produkts
1. General Information
ZINQ Technologie GmbH microZINQ® hot­dip galvanized steel
Programme holder Owner of the declaration
IBU – Institut Bauen und Umwelt e.V. ZINQ Technologie GmbH
Panoramastr. 1 An den Schleusen 6
10178 Berlin 45881 Gelsenkirchen
Germany Deutschland
Declaration number Declared product / declared unit
EPD­ZIN­20210263­IBG1­EN 1 t of microZINQ® hot­dip galvanized structural steel
This declaration is based on the product Scope:
category rules: This EPD refers to 1t of microZINQ® hot­dip
Structural steels, 11.2017 galvanized steel galvanized at the microZINQ® facility
(PCR checked and approved by the SVR) of the ZINQ® group in Hagen. Representative
foreground data collected by ZINQ Technologie GmbH
and background data from the GaBi database was
Issue date
used to conduct the LCA­study.
22.03.2022
The owner of the declaration shall be liable for the
Valid to
underlying information and evidence; the IBU shall not
21.03.2027
be liable with respect to manufacturer information, life
cycle assessment data and evidences.
The EPD was created according to the specifications
of EN 15804+A2. In the following, the standard will be
simplified as EN 15804.
Verification
The standard EN 15804 serves as the core PCR
Independent verification of the declaration and data
according to ISO 14025:2010
Dipl. Ing. Hans Peters internally x externally
(chairman of Institut Bauen und Umwelt e.V.)
Dr. Alexander Röder Matthias Klingler
(Managing Director Institut Bauen und Umwelt e.V.)) (Independent verifier)
2. Product
2.1 Product description/Product definition and heavy plates with the aforementioned zinc coating.
This EPD applies to 1 t (1000 kg) of microZINQ® hot­ The steel products are manufactured via Blast Furnace
dip galvanized structural steel which are products of with Basic Oxygen Furnace (BF+BOF) and Electric Arc
ZINQ Technologie GmbH and applied for the purpose Furnace (EAF) routes according to the EPD of
of corrosion protection of said steel components. Structural steel: Sections and Plates.
Characteristics are:
 Hot­dip zinc coating according to DIN For the placing on the market in the European
50997 consisting of a zinc­aluminium layer as Union/European Free Trade Association (EU/EFTA)
(with the exception of Switzerland) the following legal
a result of the hot­dip galvanizing process in a
provisions apply: AbZ Z-30.11-60 Mit dem
zinc­ 5 % aluminium alloy
Dünnschicht­Stückverzinkungsverfahren microZINQ®
 Applied on steel components, e.g. hot­rolled 5 feuerverzinkte Bauteile and the harmonised standard
sections or structures welded from heavy EN 10025-1: 2005 Hot rolled products of structural
plates; a typical surface of such steel steels – Part 1: General technical delivery
components per ton is 75 ­ 150 m², the conditions.The CE­marking takes into account the
proof of conformity with the respective harmonized
average value resulting from the data is 100
standards based on the legal provisions above. For the
m² per ton of product
application and use the respective national provisions
 Typical zinc­aluminium coating thickness is 5
apply.
– 15 µm, the average value resulting from the
data gathered is 12.5 µm 2.2 Application
Structural steels are intended for bolted, welded or
otherwise connected constructions of buildings or other
The EPD covers steel products of the grades S235 to
load­bearing (support) structures but also for
S960 rolled out to structural sections, merchant bars
infrastructure components, commercial vehicle
2 Environmental Product Declaration ZINQ Technologie GmbH – microZINQ(R) hot­dip galvanized steel
components and other structures. The zinc coatings Materials (zinc & auxiliaries) of the coating process:
applied to steel structures serve in particular the  Zinc alloys
purpose of protecting these against corrosive and/or  Industrial cleaner
mechanical loading during the use phase. They thus
 Corrosion inhibitor
are applied in steel applications where relevant
 Wetting agents
corrosive loadings occur and appropriate protection
against these is required to extend the service life of  Pickling additives
the steel components and ensure their functionality.  Hydrochloric acid
Zinc coatings also serve additional purposes, such as
 Hydrogen peroxide
optical design and improved fire protection.
 Ammonium hydroxide
Examples of hot­dip galvanized steel applications
include:  Flux (based on Zinc chloride and Ammonium
 Single story buildings like industrial and plus further metal chlorides, especially alkali
storage halls and alkaline earth metal chlorides))
 Multi­storey buildings like offices, residential  Caustic soda
buildings, car parks and shops  Passivation bath
 Bridges for different modes of transport like  Sealing bath
railway or roads  Binding Wire
 Sub­structure of solar panels, scaffoldings or
shelving systems Hot­dip galvanized steel is not a substance or mixture
 crash barriers, signposts and sign bridges under the chemical law (REACH). Nethertheless, the
following declaration are given for microZINQ hot­dip
galvanized steel:
 This product/article/at least one partial article
contains substances listed in the candidate
2.3 Technical Data
This EPD is valid for steel products of varied list (date: 18.12.2019) exceeding 0.1
grades and different forms of delivery according to the percentage by mass: no.
EPD of Structural steel: Sections and Plates.  This product/article/at least one partial article
contains other CMR substances in categories
Technical Data
1A or 1B which are not on the candidate list,
Name Value Unit
exceeding 0.1 percentage by mass: no.
Density 7850 kg/m3
Modulus of elasticity 210000 N/mm2  Biocide products were added to this
Coefficient of thermal expansion 12 10­6K­1 construction product or it has been treated
Thermal conductivity 48 ­ 58 W/(mK) with biocide products (this then concerns a
Melting point depending on the treated product as defined by the (EU)
1536 °C
alloy up to Ordinance on Biocide Products No.
528/2012): no.
Performance data of the product in accordance with
the declaration of performance with respect to its
essential characteristics according to EN 10025, Hot 2.6 Manufacture
rolled products of structural steels . Further product The manufacturing of structural steel refers to the
standards: ASTM A36, ASTM A283, ASTM A514, EPD of Structural steel: Sections and Plates.
ASTM A572, ASTM A573, ASTM A588, ASTM A633,
ASTM A709, ASTM A913, ASTM A992 and ASTM In hot­dip galvanizing, the fully or semi­fabricated steel
A1066. components are first cleaned using a wet­chemical
For the execution of steel structures EN 1090-2 has to pre­treatment and then coated by dipping them into
be taken into consideration. For hot­dip galvanizing the molten liquid zinc melt. This includes the use of
DIN 50997, Zinc­aluminium coatings applied by thin natural gas to fire the molten zinc to ~420°C, ensuring
film galvanizing of steel – Requirements and testing a constant temperature and compensating for thermal
has to be taken into consideration. Further relevant losses, as well as the drying furnace. Electrical energy
standards: EN ISO 14713-1, EN ISO 14713-2, ASTM is used for the extraction system at the galvanizing
A143, ASTM A153, ASTM A384, ASTM A385, ASTM kettel and for the cranes that move the galvanizing
A1072. material through the process. For this purpose, racks,
hooks, chains, wires and traverses are used in addition
2.4 Delivery status as auxiliary equipment.
The dimensions of the products declared in this EPD
may vary depending on the intended application. 2.7 Environment and health during
manufacturing
2.5 Base materials/Ancillary materials
One ton of the hot­dip galvanized structural steels During production, there are no special requirements
covered in this EPD consist of 991.08 kg of structural for safety, environmental protection and health beyond
steel according to the EPD of Structural steel: Sections the legal requirements. Compliance with these
and Plates and 8.92 kg of protective zinc coating. The requirements is verified in the course of microZINQ®
masses are based on the declared unit (100 m2 hot­dip galvanizing using management systems (ISO
surface, 12.5 µm coating thickness). 14001, ISO 45001 and ISO 50001). In addition, a
complete assessment of all substances used in the
process and duroZINQ® product, including an ABC­X
3 Environmental Product Declaration ZINQ Technologie GmbH – microZINQ(R) hot­dip galvanized steel
analysis, was carried out as part of the Cradle-to- compounds and zinc­aluminium compounds. Under
Cradle Certification process (certification has been ongoing corrosive loading of the zinc coating the zinc
valid continuously since 2016). corrodes and the layer becomes thinner over time.
This process of zinc consumption or zinc loss takes
2.8 Product processing/Installation place very slowly at a zinc corrosion rate. For
microZINQ the experience has shown a very low zinc
Processing recommendations: corrosion during utilization, which is often
Planning, processing, implementation and intended characterized by a non­linear behavior over time. The
use of microZINQ® hot­dip galvanized section and underlying mechanisms were investigated by ZINQ
plate constructions have to be carried out depending technologies GmbH in cooperation with Fraunhofer
on the respective applications according to the Institute IPA. For the present calculation a linear
generally recognized rules of engineering and corrosion rate of 0.15 µm per year is assumed, which
manufacturer’s recommendations. The standards of results from own measurements over five years in C3
EN 1993 and EN 1994 apply to the design of steel atmosphere.
structures and composite steel and concrete
structures. They include the requirements regarding 2.11 Environment and health during use
serviceability, bearing capacity, durability and fire The protective layer of the zinc coating (zinc
resistance of steel structures EN 1993 and composite carbonate, patina) formed naturally under the influence
steel and concrete structures EN 1994. of air and moisture is very stable and not soluble in
EN 1090-1 and EN 1090-2 apply to the execution of water (see 2.10) under consideration of today's
steel structures and include the requirements for strongly reduced air pollution (here especially the SO
2
factory production control. In addition, these European concentration in the air) and proper application (no
Standards will work in connection with national water drainage permanently provided by the design).
amendments, national instructions, guidelines and The zinc ion runoff significantly depends on the load of
publications, as well as legal provisions. "acidic" air pollutants, especially SO . As the SO
2 2
Regarding transport and storage of microZINQ® hot­ concentration in the air has decreased to one­fifth of
dip galvanized sections and plates, the generally previous levels over the past 30 years, there has also
accepted requirements for securing loads have to be been a corresponding decrease in the zinc runoff and
observed. thus of the zinc concentration in precipitation water.
Instruction details of the manufacturer based on The legal limits for the total concentration of zinc in
verified standards and guidelines e.g. regarding drinking water are undercut. In water systems, only a
welding, bolting, hot and cold forming or assembly are small portion of the total zinc concentration is available
to be observed in every case. to an organism; this amount is called the biologically
available amount. It is related to the physicochemical
Occupational safety/Environmental protection: conditions of the receiving water body. For example,
When processing/using microZINQ® hot­dip bioavailability is affected by the amount of zinc that is
galvanized steel sections and plates pursuant to the organically or inorganically bound, bound to particles,
generally recognized rules of engineering there are no or competing with other ions.
measures to be taken which are going beyond the There are no known adverse effects on health when
public occupational health and safety. steel hot­dip galvanized with microZINQ® is used as
The processing/using of microZINQ® hot­dip intended. Like iron, zinc is one of the metals essential
galvanized steel sections and plates pursuant to the for life. Zinc is not accumulated in the body. The zinc
generally recognized rules of engineering does not intake recommendation of the German Nutrition
release substantial environmental pollutants. Particular Society (DGE) is 15 mg daily.
measures to protect the environment are not required.
Residual material: 2.12 Reference service life
During microZINQ® hot­dip galvanizing as well as Structural steel products are supposed to serve at
during processing of microZINQ® hot­dip galvanized least the lifetime of a building which is 50 years
steel residual pieces as well as turnings are to be according to EN 15978. The technical service life of a
separately collected. Zinc­rich waste from the galvanized steel product is determined by the time the
microZINQ® hot­dip galvanizing process is treated and protecting zinc coating stays on the steel to protect it
returned to the zinc cycle. microZINQ® hot­dip from corrosion. At a rate of 0.15 μm per year (section
galvanized scrap steel is entirely recycled by melting 2.10) this leads to a technical service life of at least 83
and producing new steel products. years and therefore exceeds the 50 years lifetime of
buildings.
2.9 Packaging
No additional packaging is necessary since
the microZINQ® coating provides the protecting 2.13 Extraordinary effects
function of a package.
Fire
The material is class A1, i.e. not flammable per EN
2.10 Condition of use 13501.
microZINQ® hot­dip galvanized steel products are Under fire load, the zinc coating has a positive effect
non­/low­alloyed steel products with a protective on the steel structure in that it slows down its heating,
coating, which results from hot­dip galvanizing in a zinc which ensures the load­bearing capacity of the
melt of nominal 95 mass% zinc, the rest being structure for a longer period of time compared to
aluminium and minor alloying elements. ungalvanized, unprotected steel.
During use the zinc coatings undergo permanent When heated above 650°C, the thin zinc coating
reactions with its atmosphere, building a very resistant evaporates briefly as zinc oxide (ZnO), producing
layer of zinc carbonate (carbonisation), aluminium smoke. The ZnO smoke, inhaled over a longer period
4 Environmental Product Declaration ZINQ Technologie GmbH – microZINQ(R) hot­dip galvanized steel
of time, can cause "zinc fever" (diarrhoea, fever, dry
throat), which, however, disappears completely some 2.14 Re-use phase
days after inhalation. Steel sections and plates made of microZINQ® hot­dip
galvanized steels are recyclable to 100 % EPD of
Structural Steel: Sections and Plates. Re­use takes
Brandschutz place for around 11 % of the products while 88 % are
Name Value recycled in a closed loop. Around 1 % can not be
Building material class A1 regained due to occurring losses. The zinc coating is
carbonized over the lifetime of the steel structure.
Water
Under the influence of water, no negative effects on 2.15 Disposal
the functional capability of microZINQ hot­dip Due to its high value as a raw material, hot­dip
galvanized steel within the intended service life are to galvanized steel scrap is not disposed of but recycled
be expected ­ provided that it is used as intended. in a long­established cycle. Reaction products of the
zinc coating with the atmosphere (zinc carbonate
Mechanical destruction resulting from carbonization) are removed from the
Due to the ductility of steel and the high mechanical surface in very low concentrations over the lifespan of
resistance of the microZINQ® hot­dip zinc the steel product, but without known harm to the
coating, microZINQ® hot­dip steel structures react environment.
resiliently in the event of unforeseeable mechanical Waste code according to European Waste Catalogue
destruction. In case of tensile load, necking will occur EWC:
before cracking. In case of lasting high compression 17 04 05 ­ iron and steel
load, components of microZINQ® hot­dip galvanized
steel may buckle or bulge. No splintering or breaking 2.16 Further information
edges shall result. Further information on microZINQ® products can be
obtained from www.zinq.com.
3. LCA: Calculation rules
3.1 Declared Unit been accounted for using a German average grid mix.
The declared unit is 1t (1000 kg) of hot­dip galvanized The proportion of green electricity demand for the
structural steel. Data from the microZINQ® facility of galvanizing process is 100 %. Therefore, no residual
the ZINQ® group in Hagen as a representative grid mix has been considered.
production site has been used to declare a
representative product (100 m2 surface, 12.5 µm Module B1-B7 consider the following:
coating thickness).  Carbonisation of the Zinc coating during use
of the product. This serves as a carbon
Declared Unit
dioxide sink. The calculation is based on the
Name Value Unit
stoichiometric ratio lowered by an amount to
Declared unit 1 t
account for real conditions.
 during intended use over the considered
lifetime of hot­dip galvanized structural steels,
3.2 System boundary no maintenance, replacement or
Type of the EPD: Cradle to gate with options,modules refurbishment is needed. The products do not
C1–C4, and module D.
use energy or water.
Modules A1­A4, B1­B7, C1­C4 and D have been
considered.
Module C1-C4 consider the following:
Module A1-A4 consider the following:  Deconstruction of structural steel,
 Production of structural steel according to the  transport to the end­of­life,
EPD of Structural Steel: Sections and Plates,  processing and disposal according to the
 production of zinc and zinc alloy EPD of Structural Steel: Sections and Plates.
components,
 transport of the structural steel to the Due to carbonisation, no remaining zinc must be
manufacturing sites, considered.
 the galvanizing process, including all
auxiliaries and the use of electricity and Module D considers benefits and loads beyond the
system boundary according to the EPD of Structural
thermal energy,
Steel: Sections and Plates.,
 transport from the manufacturing sites to the
construction site. 3.3 Estimates and assumptions
Primary data was used to model all on­site processes
For the electricity consumption of the galvanizing of the hot­dip galvanizing process. Data were cross­
process a renewable energy grid mix has been taken checked to identify and eliminate data gaps. High­
into account. The electricity usage of the production of quality secondary data from the GaBi database was
steel as well as module D refers to to the EPD of used to model upstream material and energy flows.
Structural Steel: Sections and Plates. Electricity credits Secondary data was as technologically and
of energy recovery inside the system boundaries have geographically representative as possible. Zn/Al
5 Environmental Product Declaration ZINQ Technologie GmbH – microZINQ(R) hot­dip galvanized steel
master alloys, alloying elements and auxiliaries are productions plants.
considered using their material weights. Instead of All relevant background datasets are taken from the
primary data collection from suppliers to reflect specific GaBi database. The study is based on high
brand products, datasets from the GaBi database for quality data.
standard processing chemicals have been used.
For sludges, a solid waste content was assumed. This 3.7 Period under review
solid waste content is handled as hazardous waste Allocation for the structural steel is done according to
with the respective treatment. Waste water and water the EPD of Structural Steel: Sections and plates. The
content of the sludges are assumed to be treated in hot dip galvanizing process does not deliver any co­
municipal waste water treatment. Other wastes are products. The applied model does not contain any
treated as commercial waste in a municipal waste allocation.
incineration plant.
3.8 Allocation
The allocations of relevance for calculation
3.4 Cut-off criteria (appropriation of expenses across various products)
No cut­off criteria are applied in this study. All reported must be indicated,
data were incorporated and modelled using the best at least:
available LCI data. Data for the sites were cross­  Allocation of energy, auxiliary and operating
checked with one another to identify potential data materials used for individual products in a
gaps. No processes, materials or emissions that are factory;
known to make a significant contribution to the  Allocation of co­production processes;
environmental impact of the products studied have  Allocation in the use of recycled and/or
been omitted. On this basis, there is no evidence to secondary raw materials;
suggest that input or outputs contributing more than 1  Loads and benefits beyond the system
% to the overall mass or energy of the system or that boundary from recycling or energy recovery of
are environmentally significant have been omitted. It packaging materials and production waste;
can be assumed, that all excluded flows contribute less
 Loads and benefits beyond the system
than 5 % to the impact assessment categories.
boundary from recycling or energy recovery
Production of capital equipment, facilities and
from the end of life of the product.
infrastructure required for manufacture are outside the
scope of this assessment.
whereby reference must be made to the modules in
Transport of base materials with low shares in the
which the allocations are performed.
composition are neglected.
3.9 Comparability
Basically, a comparison or an evaluation of EPD data
3.5 Background data
is only possible if all the data sets to be compared
The LCA model is created using the GaBi
were created according to EN 15804 and the building
Software system for life cycle engineering, developed
context, respectively the product­specific
by Sphera Solutions GmbH. The GaBi
characteristics of performance, are taken into account.
database provides the life cycle inventory data for
several of the raw and process materials obtained from
The GaBi database provides the life cycle inventory
the background system. The most recent of the
data for several of the raw and process materials
database was 2020.
obtained from the background system. The most
recent of the database was 2020.
3.6 Data quality
The foreground data collected by ZINQ Technologie
GmbH are based on yearly production amounts in
4. LCA: Scenarios and additional technical information
Characteristic product properties Name Value Unit
Information on biogenic Carbon Reuse 109 kg
Recycling 872 kg
Energy recovery 0 kg
Landfilling 9.9 kg
The production of the steel refers to the EPD of
Structural Steel: Sections and Plates.
Information for the scenario used is given in the
following tables. Information regarding the service life
is given in section 2.12.
Transport to Construction site (A4)
Name Value Unit
Transport distance 100 km
Capacity utilisation (including
61 %
empty runs)
Ende des Lebenswegs (C1-C4)
6 Environmental Product Declaration ZINQ Technologie GmbH – microZINQ(R) hot­dip galvanized steel
5. LCA: Results
Disclaimer:
EP­freshwater: This indicator has been calculated as “kg P eq” as required in the characterization model
(EUTREND model, Struijs et al., 2009b, as implemented in ReCiPe;
http://eplca.jrc.ec.europa.eu/LCDN/developerEF.xhtml).
DESCRIPTION OF THE SYSTEM BOUNDARY (X = INCLUDED IN LCA; ND = MODULE OR INDICATOR NOT
DECLARED; MNR = MODULE NOT RELEVANT)
BENEFITS AND
CONSTRUCTI LOADS
PRODUCT STAGE ON PROCESS USE STAGE END OF LIFE STAGE BEYOND THE
STAGE SYSTEM
BOUNDARIES
7 Environmental Product Declaration ZINQ Technologie GmbH – microZINQ(R) hot­dip galvanized steel
lairetam
waR
ylppus tropsnarT
gnirutcafunaM
eht
morf
tropsnarT
etis
eht
ot
etag
ylbmessA esU
ecnanetniaM
riapeR
tnemecalpeR tnemhsibrufeR
ygrene
lanoitarepO esu
retaw
lanoitarepO esu
noitcurtsnoc­eD
noitilomed tropsnarT
gnissecorp
etsaW
lasopsiD ­esueR ­yrevoceR ­gnilcyceR laitnetop
A1 A2 A3 A4 A5 B1 B2 B3 B4 B5 B6 B7 C1 C2 C3 C4 D
X X X X ND X X X X X X X X X X X X
RESULTS OF THE LCA - ENVIRONMENTAL IMPACT according to EN 15804+A2: declared unit and
product
Core Indicator Unit A1 A2 A3 A4 B1 B2 B3 B4 B5 B6 B7 C1 C2 C3 C4 D
­ ­
1.21E+2.99E+1.59E+6.03E+ 0.00E+0.00E+0.00E+0.00E+0.00E+0.00E+1.11E+2.99E+1.77E+0.00E+
GWP­total [kg CO2­Eq.]
3 1 2 0
2.00E+
0 0 0 0 0 0 1 0 0 0
3.77E+
0 2
­ ­
1.21E+2.97E+1.58E+5.99E+ 0.00E+0.00E+0.00E+0.00E+0.00E+0.00E+1.11E+2.97E+1.78E+0.00E+
GWP­fossil [kg CO2­Eq.]
3 1 2 0
2.00E+
0 0 0 0 0 0 1 0 0 0
3.76E+
0 2
1.90E+­5.08E­8.75E­­1.03E­0.00E+0.00E+0.00E+0.00E+0.00E+0.00E+0.00E+3.69E­­5.08E­­1.38E­0.00E+­3.68E­
GWP­biogenic [kg CO2­Eq.]
0 2 1 2 0 0 0 0 0 0 0 2 3 2 0 1
3.45E­ 2.41E­ 1.47E­ 4.86E­0.00E+0.00E+0.00E+0.00E+0.00E+0.00E+0.00E+1.61E­ 2.41E­ 3.21E­0.00E+­3.00E­
GWP­luluc [kg CO2­Eq.]
1 1 2 2 0 0 0 0 0 0 0 2 2 3 0 2
­9.15E­3.58E­ 3.28E­ 7.21E­0.00E+0.00E+0.00E+0.00E+0.00E+0.00E+0.00E+2.44E­ 3.58E­ 3.30E­0.00E+2.81E­
ODP [kg CFC11­Eq.]
8 15 8 16 0 0 0 0 0 0 0 13 16 14 0 13
3.21E+3.05E­ 1.03E­ 6.16E­0.00E+0.00E+0.00E+0.00E+0.00E+0.00E+0.00E+2.45E­ 3.05E­ 5.09E­0.00E+­8.67E­
AP [mol H+­Eq.]
0 2 1 3 0 0 0 0 0 0 0 2 3 3 0 1
5.28E­ 9.04E­ 2.00E­ 1.82E­0.00E+0.00E+0.00E+0.00E+0.00E+0.00E+0.00E+2.96E­ 9.04E­ 4.53E­0.00E+­1.92E­
EP­freshwater [kg P­Eq.]
4 5 4 5 0 0 0 0 0 0 0 5 6 6 0 4
7.48E­ 8.89E­ 2.82E­ 1.79E­0.00E+0.00E+0.00E+0.00E+0.00E+0.00E+0.00E+5.43E­ 8.89E­ 1.36E­0.00E+­1.73E­
EP­marine [kg N­Eq.]
1 3 2 3 0 0 0 0 0 0 0 3 4 3 0 1
­
8.16E+1.07E­ 3.37E­ 2.16E­0.00E+0.00E+0.00E+0.00E+0.00E+0.00E+0.00E+5.71E­ 1.07E­ 1.46E­0.00E+
EP­terrestrial [mol N­Eq.] 1.81E+
0 1 1 2 0 0 0 0 0 0 0 2 2 2 0
0
2.50E+2.47E­ 1.58E­ 4.98E­0.00E+0.00E+0.00E+0.00E+0.00E+0.00E+0.00E+1.49E­ 2.47E­ 3.82E­0.00E+­6.64E­
POCP [kg NMVOC­Eq.]
0 2 1 3 0 0 0 0 0 0 0 2 3 3 0 1
4.70E­ 2.13E­­1.57E­4.30E­0.00E+0.00E+0.00E+0.00E+0.00E+0.00E+0.00E+3.21E­ 2.13E­ 4.53E­0.00E+­4.04E­
ADPE [kg Sb­Eq.]
3 6 3 7 0 0 0 0 0 0 0 6 7 7 0 3
­
1.29E+3.96E+2.57E+7.99E+0.00E+0.00E+0.00E+0.00E+0.00E+0.00E+0.00E+1.95E+3.96E+2.99E+0.00E+
ADPF [MJ] 3.50E+
4 2 3 1 0 0 0 0 0 0 0 2 1 1 0
3
­ ­
[m³ world­Eq 4.67E+2.66E­ 5.37E­0.00E+0.00E+0.00E+0.00E+0.00E+0.00E+0.00E+2.42E+2.66E­ 3.38E­0.00E+
WDP 1.17E+ 3.35E+
deprived] 2 1 2 0 0 0 0 0 0 0 0 2 1 0
2 1
GWP = Global warming potential; ODP = Depletion potential of the stratospheric ozone layer; AP = Acidification potential of land and water; EP =
Caption Eutrophication potential; POCP = Formation potential of tropospheric ozone photochemical oxidants; ADPE = Abiotic depletion potential for non­
fossil resources; ADPF = Abiotic depletion potential for fossil resources; WDP = Water (user) deprivation potential
RESULTS OF THE LCA - INDICATORS TO DESCRIBE RESOURCE USE according to EN 15804+A2:
declared unit and product
Indicator Unit A1 A2 A3 A4 B1 B2 B3 B4 B5 B6 B7 C1 C2 C3 C4 D
PERE [MJ] 1310.00 22.30 1160.00 4.49 0.00 0.00 0.00 0.00 0.00 0.00 0.00 86.40 2.23 11.90 0.00 38.30
PERM [MJ] ND ND ND ND 0.00 0.00 0.00 0.00 0.00 0.00 0.00 ND ND ND 0.00 ND
PERT [MJ] 1310.00 22.30 1160.00 4.49 0.00 0.00 0.00 0.00 0.00 0.00 0.00 86.40 2.23 11.90 0.00 38.30
12900.0 ­
PENRE [MJ] 396.00 2570.00 80.00 0.00 0.00 0.00 0.00 0.00 0.00 0.00 195.00 39.60 29.90 0.00
0 3500.00
PENRM [MJ] 0.00 0.00 0.00 0.00 0.00 0.00 0.00 0.00 0.00 0.00 0.00 0.00 0.00 0.00 0.00 0.00
12900.0 ­
PENRT [MJ] 396.00 2570.00 80.00 0.00 0.00 0.00 0.00 0.00 0.00 0.00 195.00 39.60 29.90 0.00
0 3500.00
SM [kg] 820.00 0.00 0.00 0.00 0.00 0.00 0.00 0.00 0.00 0.00 0.00 0.00 0.00 0.00 0.00 0.00
RSF [MJ] 0.00 0.00 0.00 0.00 0.00 0.00 0.00 0.00 0.00 0.00 0.00 0.00 0.00 0.00 0.00 0.00
NRSF [MJ] 0.00 0.00 0.00 0.00 0.00 0.00 0.00 0.00 0.00 0.00 0.00 0.00 0.00 0.00 0.00 0.00
FW [m³] 11.30 0.03 ­2.67 0.01 0.00 0.00 0.00 0.00 0.00 0.00 0.00 0.10 0.00 0.01 0.00 ­0.82
PERE = Use of renewable primary energy excluding renewable primary energy resources used as raw materials; PERM = Use of
renewable primary energy resources used as raw materials; PERT = Total use of renewable primary energy resources; PENRE = Use of
non­renewable primary energy excluding non­renewable primary energy resources used as raw materials; PENRM = Use of non­
Caption
renewable primary energy resources used as raw materials; PENRT = Total use of non­renewable primary energy resources; SM = Use
of secondary material; RSF = Use of renewable secondary fuels; NRSF = Use of non­renewable secondary fuels; FW = Use of net fresh
water
RESULTS OF THE LCA – WASTE CATEGORIES AND OUTPUT FLOWS according to EN 15804+A2:
declared unit and product
Indicator Unit A1 A2 A3 A4 B1 B2 B3 B4 B5 B6 B7 C1 C2 C3 C4 D
HWD [kg] 1.28E­41.84E­5­2.75E­53.72E­60.00E+00.00E+00.00E+00.00E+00.00E+00.00E+00.00E+08.07E­81.84E­61.17E­70.00E+0­2.74E­4
NHWD [kg] 9.64 0.06 3.76 0.01 0.00 0.00 0.00 0.00 0.00 0.00 0.00 0.14 0.01 9.94 0.00 25.00
RWD [kg] 5.79E­14.91E­4­6.51E­39.90E­50.00E+00.00E+00.00E+00.00E+00.00E+00.00E+00.00E+02.96E­24.91E­53.96E­30.00E+0­6.00E­2
CRU [kg] 0.00 0.00 0.00 0.00 0.00 0.00 0.00 0.00 0.00 0.00 0.00 0.00 0.00 0.00 0.00 0.00
MFR [kg] 0.00 0.00 0.00 0.00 0.00 0.00 0.00 0.00 0.00 0.00 0.00 0.00 0.00 109.00 0.00 0.00
MER [kg] 0.00 0.00 0.00 0.00 0.00 0.00 0.00 0.00 0.00 0.00 0.00 0.00 0.00 872.00 0.00 0.00
EEE [MJ] 0.00 0.00 0.00 0.00 0.00 0.00 0.00 0.00 0.00 0.00 0.00 0.00 0.00 0.00 0.00 0.00
EET [MJ] 0.00 0.00 0.00 0.00 0.00 0.00 0.00 0.00 0.00 0.00 0.00 0.00 0.00 0.00 0.00 0.00
HWD = Hazardous waste disposed; NHWD = Non­hazardous waste disposed; RWD = Radioactive waste disposed; CRU = Components
Caption for re­use; MFR = Materials for recycling; MER = Materials for energy recovery; EEE = Exported electrical energy; EEE = Exported
thermal energy
RESULTS OF THE LCA – additional impact categories according to EN 15804+A2-optional:
[declared unit and product]
Indicator Unit A1 A2 A3 A4 B1 B2 B3 B4 B5 B6 B7 C1 C2 C3 C4 D
[Disease 0.00E+ 0.00E+ 0.00E+ 0.00E+ 0.00E+ 0.00E+ 0.00E+ 0.00E+ ­1.13E­
PM 3.20E­51.82E­72.78E­73.67E­8 2.05E­71.82E­84.99E­8
Incidence] 0 0 0 0 0 0 0 0 5
­
[kBq U235­ 1.08E+ ­8.30E­ 0.00E+ 0.00E+ 0.00E+ 0.00E+ 0.00E+ 0.00E+ 0.00E+ 4.85E+ 0.00E+
IRP 7.09E­2 1.43E­2 7.09E­36.48E­1 6.77E+
Eq.] 2 1 0 0 0 0 0 0 0 0 0
0
­ ­
7.72E+ 2.80E+ 5.65E+ 0.00E+ 0.00E+ 0.00E+ 0.00E+ 0.00E+ 0.00E+ 0.00E+ 8.33E+ 2.80E+ 1.39E+ 0.00E+
ETP­fw [CTUe] 1.09E+ 3.12E+
3 2 1 0 0 0 0 0 0 0 1 1 1 0
3 2
­1.55E­ 0.00E+ 0.00E+ 0.00E+ 0.00E+ 0.00E+ 0.00E+ 0.00E+ 5.86E­ 5.14E­ 0.00E+
HTP­c [CTUh] 2.67E­75.86E­9 1.18E­9 2.30E­9 6.61E­8
8 0 0 0 0 0 0 0 10 10 0
­4.36E­ 0.00E+ 0.00E+ 0.00E+ 0.00E+ 0.00E+ 0.00E+ 0.00E+ 0.00E+ ­4.32E­
HTP­nc [CTUh] 2.42E­53.02E­7 6.10E­8 8.48E­83.02E­83.17E­8
8 0 0 0 0 0 0 0 0 6
­
8.26E+ 1.39E+ 6.09E+ 2.80E+ 0.00E+ 0.00E+ 0.00E+ 0.00E+ 0.00E+ 0.00E+ 0.00E+ 6.20E+ 1.39E+ 9.30E+ 0.00E+
SQP [­] 3.30E+
2 2 1 1 0 0 0 0 0 0 0 1 1 0 0
1
PM = Potential incidence of disease due to PM emissions; IR = Potential Human exposure efficiency relative to U235; ETP­fw = Potential
Caption comparative Toxic Unit for ecosystems; HTP­c = Potential comparative Toxic Unit for humans (cancerogenic); HTP­nc = Potential
comparative Toxic Unit for humans (not cancerogenic); SQP = Potential soil quality index
6. LCA: Interpretation
The interpretation of this EPD highlights the different impact categories.
contribution of the hot­dip galvanizing process in the Negative contributions of module A3 (the hot­dip
environmental impact of 1 t of microZINQ® hot­dip galvanizing process) for ADPE and WDP are linked to
galvanized steel. While the highest share of impacts as the recovery of high­value zinc, a sulphidic ore, using a
for a hot­dip galvanized product is related to the rotary kiln while the upstream of zinc is part of module
production of the structural steel as part of Module A1, A1. This results in a net negative value of module A3
this refers to the EPD of Structural Steel: Sections for impact categories linked to the mining of zinc.
and Plates. The potential benefits in module D are The results show a similar trend to GWP for most of
exclusively attributable to the steel. Additionally, the the impact categories Module A1 is linked to the
use phase serves as a sink for CO due to highest impacts and module D offers benefits to reuse
2
carbonization of the zinc coating. The following graph and recycling of the structural steel.
shows the relative contribution of each module for the
8 Environmental Product Declaration ZINQ Technologie GmbH – microZINQ(R) hot­dip galvanized steel
7. Requisite evidence
7.1 Weathering performance industrial atmosphere with moderate sulfur dioxide
The corrosion rate of zinc and zinc­aluminium load and a coastal atmosphere with low salt load and
compounds depend on the position of the component thus corresponds to the typical corrosive load of steel
and the conditions of the surrounding atmosphere structures, the corrosion rate is assumed to be 0.15
(corrosivity categories for zinc according to EN ISO µm/year.
12944-2). For corrosivity category C3, which according
to this standard is characteristic of an urban and
8. References
Standards ASTM A384 / A384M: 2019 Standard Practice for
Safeguarding Against Warpage and Distortion During
ASTM A36 Hot­Dip Galvanizing of Steel Assemblies
ASTM A36 / A36M: 2019 Standard Specification for
Carbon Structural Steel ASTM A385
ASTM A385 / A385M: 2020 Standard Practice for
ASTM A123 Providing High­Quality Zinc Coatings (Hot­Dip)
ASTM A123 / A123M: 2017 Standard Specification for
Zinc (Hot­Dip Galvanized) Coatings on Iron and Steel ASTM A514
Products ASTM A514 / A514M: 2018 Standard Specification for
High­Yield­Strength, Quenched and Tempered Alloy
ASTM A143 Steel Plate
ASTM A143 / A143M: 2020 Standard Practice for
Safeguarding Against Embrittlement of Hot­Dip ASTM A572
Galvanized Structural Steel Products and Procedure ASTM A572 / A572M: 2021 Standard Specification for
for Detecting Embrittlement High­Strength Low­Alloy Columbium­Vanadium
Structural Steel
ASTM A153
ASTM A153 / A153M: 2016 Standard Specification for ASTM A573
Zinc Coating (Hot­Dip) on Iron and Steel Hardware ASTM A573 / A573M: 2020 Standard Specification for
Structural Carbon Steel Plates
ASTM A283
ASTM A283 / A283M: 2018 Standard Specification for ASTM A588
Low and Intermediate Tensile Strength Carbon Steel ASTM A588 / A588M: 2019 Standard Specification for
Plates High­Strength Low­Alloy Structural Steel, up to 50 ksi
[345 MPa] Minimum Yield Point, with Atmospheric
ASTM A384 Corrosion Resistance
9 Environmental Product Declaration ZINQ Technologie GmbH – microZINQ(R) hot­dip galvanized steel
EN 13501­1:2018 Fire classification of construction
ASTM A633 products and building elements Classification using
ASTM A633 / A633M: 2018 Standard Specification for data from reaction to fire tests
Normalized High­Strength Low­Alloy Structural Steel
Plates EN 14025
DIN EN ISO 14025:2010 Environmental labels and
ASTM A709 declarations. Type III environmental declarations.
ASTM A709 / A709M: 2018 Standard Specification for Principles and procedures
Structural Steel for Bridges
EN ISO 14713-1
ASTM A913 EN ISO 14713­1: 2017 Zinc coatings ­ Guidelines and
ASTM A913 / A913M: 2019 Standard Specification for recommendations for the protection against corrosion
High­Strength Low­Alloy Steel Shapes of Structural of iron and steel in structures ­ Part 1: General
Quality, Produced by Quenching and Self­Tempering principles of design and corrosion resistance
Process (QST)
EN ISO 14713-2
ASTM A992 EN ISO 14713­2:2020 Zinc coatings ­ Guidelines and
ASTM A992 / A992M: 2020 Standard Specification for recommendations for the protection against corrosion
Structural Steel Shapes of iron and steel in structures ­ Part 2: Hot dip
galvanizing
ASTM A1066
ASTM A1066 / A1066M: 2015 Standard Specification EN 15804
for High­Strength Low­Alloy Structural Steel Plate EN 15804+A2 Sustainability of construction works ­
Produced by Thermo­Mechanical Controlled Process Environmental product declarations ­ Core rules for the
(TMCP) product category of construction products
ASTM A1027 EN 15978
ASTM A1072 / A1072M: 2015 Standard Specification DIN EN 15978
for Zinc­5% Aluminum (Hot­Dip) Coatings on Iron and Sustainability of construction works ­ Assessment of
Steel Products environmental performance of buildings ­ Calculation
method
DIN EN ISO 12944-2
DIN EN ISO 12944­2 Paints and varnishes ­ Corrosion ISO 14001
protection of steel structures by protective paint ISO 14001:2015 Environmental management
systems ­ Part 2: Classification of environments systems ­ Requirements with guidance for use
DIN 50997 ISO 45001
DIN 50997:2020 Zinc­aluminium coatings applied by ISO 45001: 2018 Occupational health and safety
thin film galvanizing of steel ­ Requirements and management systems ­ Requirements with guidance
testing for use
EN 1090-1 ISO 50001
EN 1090­1:2012 Execution of steel structures and ISO 5001:2018 Energy management systems ­
aluminium structures ­ Part 1: Requirements for Requirements with guidance for use
conformity assessment of structural components
EN 1090-2 Further references
EN 1090­2:2018 Execution of steel structures and
aluminium structures ­ Part 2: Technical requirements AbZ Z30.11-60
for steel structures Allgemeine bauaufsichtliche Zulassung/Allgemeine
Bauartgenehmigung Z­30.11­60 10:2020 Mit dem
EN 1993 Dünnschicht­Stückverzinkungsverfahren microZINQ®
EN 1993 Eurocode 3 ­ Design of steel structures 5 feuerverzinkte Bauteile
EN 1994 Cradle-to-Cradle Certification
EN 1994 Eurocode 4: Design of composite steel and Guidance for the Cradle to Cradle Certified™ Product
concrete structures Standard, Cradle to Cradle Products Innovation
Institute www.c2ccertified.com
EN ISO 1461
EN ISO 1461:2009 Hot dip galvanized coatings on EPD of Structural Steel: Sections and Plates
fabricated iron and steel articles ­ Specifications and Environmental Product Declaration: Structural Steel:
test methods Sections and Plates. bauforumstahl e.V., EPD­BFS­
20180116­IBG2­EN. Berlin: Institut Bauen und Umwelt
EN 10025 e.V. (ed.), 25.10.2018.
EN 10025 Hot rolled products of structural steels
EWC
EN 10025-1 European Waste Catalogue, established by
EN 10025­1: 2005 Hot rolled products of structural Commission decision 2000/532/EC2
steels – Part 1: General technical delivery conditions
GaBi Database
EN 13501
10 Environmental Product Declaration ZINQ Technologie GmbH – microZINQ(R) hot­dip galvanized steel
Sphera Solutions GmbH. (2020). GaBi LCA Database Bauen und Umwelt e.V., 2021. www.ibu­epd.com
Documentation. Retrieved from
gabi.sphera.com/international/support/gabi/ PCR Part A
Calculation Rules for the Life Cycle Assessment and
GaBi Software Requirements on the Project Report according to EN
Sphera Solutions GmbH. (2020). GaBi Software. For 15804+A2:2. Institut Bauen und Umwelt e.V. (IBU).
further information see: November 2021. www.ibu­epd.com
gabi.sphera.com/international/index/
PCR Part B
German Nutrition Society (DGE) Requirements on the EPD for www.ibu­epd.com
German Nutrition Society / Deutsche Gesellschaft für Structural steels. Institut Bauen und Umwelt e.V. (IBU).
Ernäherung e.V. (DGE), reference values for Nutrient November 2021. www.ibu­epd.com
intake, www.dge.de
IBU 2021
General Instructions for the EPD programme of Institut
Bauen und Umwelt e.V. Version 2.0, Berlin: Institut
11 Environmental Product Declaration ZINQ Technologie GmbH – microZINQ(R) hot­dip galvanized steel
Publisher
Institut Bauen und Umwelt e.V. Tel +49 (0)30 3087748­ 0
Panoramastr. 1 Fax +49 (0)30 3087748­ 29
10178 Berlin Mail info@ibu­epd.com
Germany Web www.ibu-epd.com
Programme holder
Institut Bauen und Umwelt e.V. Tel +49 (0)30 ­ 3087748­ 0
Panoramastr 1 Fax +49 (0)30 – 3087748 ­ 29
10178 Berlin Mail info@ibu­epd.com
Germany Web www.ibu-epd.com
Author of the Life Cycle
Assessment Tel +49 711 341817­0
Sphera Solutions GmbH Fax +49 711 341817­25
Hauptstraße 111­ 113 Mail info@sphera.com
70771 Leinfelden­Echterdingen Web www.sphera.com
Germany
Sphera Solutions GmbH Tel +49 711 341817­0
Hauptstr. 111­113 Fax +49 711 341817­25
70771 Leinfelden­Echterdingen https://sphera.com/
Germany
ZINQ Technologie GmbH Tel +49 209 9403400
An den Schleusen 6 Fax +49 209 9403444
45881 Gelsenkirchen Mail thomas.pinger@zinq.com
Germany Web www.zinq.com
Owner of the Declaration
ZINQ Technologie GmbH Tel +49 209 9403400
An den Schleusen 6 Fax +49 209 9403444
45881 Gelsenkirchen Mail thomas.pinger@zinq.com
Germany Web www.zinq.com
