ENVIRONMENTAL PRODUCT DECLARATION
as per ISO 14025 and EN 15804+A1
Owner of the Declaration Sto SE & Co. KGaA
Programme holder Institut Bauen und Umwelt e.V. (IBU)
Publisher Institut Bauen und Umwelt e.V. (IBU)
Declaration number EPD-IWM-STO-20210129-IBG1-DE
Issue date 07.07.2021
Valid to 06.07.2026
Mineral pre-made mortar: rendering mortar –
normal/finishing render with special properties
Sto SE & Co. KGaA
www.ibu-epd.com | https://epd-online.com
Umwelt Produktdeklaration Name des Herstellers – Name des Produkts
1. General Information
Sto SE & Co. KGaA Rendering mortar – normal/finishing
render with special properties
Programme holder Owner of the declaration
IBU – Institut Bauen und Umwelt e.V. Sto SE & Co. KGaA
Panoramastr. 1 Ehrenbachstraße 1
10178 Berlin D-79780 Stühlingen
Germany Germany
Declaration number Declared product / declared unit
EPD-IWM-STO-20210129-IBG1-DE 1 kg rendering mortar as a mineral pre-made mortar,
normal/finishing render product group with special
properties and a dry bulk density greater than 1300
kg/m³ and less than 1800 kg/m³.
Product names:
Sto-Baukleber, Sto Byggklister, Sto Byggklister, Sto
Byggeklæber, Sto Liimalaasti, (DE, SE, NO, DK, FI);
StoLevell Cote F 0-1 mm, (DE, SE, NO, DK, FI);
StoLevell Cote F 0-3 mm, (DE, SE,NO, DK, FI);
This declaration is based on the product Scope:
category rules: This document is a model EPD. When calculating the
Mineral factory-made mortar, 11.2017 Life Cycle Assessment, the product selected to
(PCR checked and approved by the SVR) represent the group in question was the product with
the highest environmental impact in that group. This
EPD applies exclusively to rendering and plastering
Issue date
mortars – normal/finishing render or plaster with
07.07.2021
special properties as mineral pre-made mortars for
association members; these can be found on the
Valid to association’s website. Any numerical values – e.g. for
06.07.2026 constructional data or concentration specifications –
are average values that are customary in practice for
this product group.
The owner of the declaration shall be liable for the
underlying information and evidence; the IBU shall not
be liable with respect to manufacturer information, life
cycle assessment data and evidences.
The EPD was created according to the specifications
of EN 15804+A1. In the following, the standard will be
simplified as EN 15804.
Verification
The standard EN 15804 serves as the core PCR
Independent verification of the declaration and data
according to ISO 14025:2010
Dipl. Ing. Hans Peters internally x externally
(chairman of Institut Bauen und Umwelt e.V.)
Dr. Alexander Röder Matthias Schulz
(Managing Director Institut Bauen und Umwelt e.V.)) (Independent verifier)
2. Product
2.1 Product description/Product definition Mineral rendering and plastering mortars are mixtures
Mineral pre-made mortars are mortars whose of one or more mineral binders, aggregates, water, and
components are mixed at the factory and not on the – if applicable – additions or admixtures for the
construction site. They are divided into three different manufacture of renders or plasters. Rendering and
types – masonry mortar, rendering and plastering plastering mortars are applied to walls and ceilings in
mortar, and screed material – depending on the type of one or more layers as required. Alongside the
application. aesthetic design of the surface, they protect against
effects of the weather when used as external renders
2 Environmental Product Declaration Sto SE & Co. KGaA – Mineral pre-made mortar: rendering and plastering mortar –
normal/finishing render or plaster with special properties
and provide an even substrate for paint coats and 2.4 Delivery status
wallpaper when used as internal plasters. In the case Mineral rendering and plastering mortars –
of reinforced concrete ceilings and stairs, normal/finishing render or plaster with special
renders/plasters also serve as fire protection; when properties are produced and delivered as pre-made
porous aggregates are added, they serve as thermal dry mortars. Pre-made dry mortar is a mortar made
protection. Depending on the technical data, the base from raw materials that are placed into containers dry
materials and processing aids used, and the practical at the factory, delivered to the construction site, and
application, rendering and plastering mortars are then mixed with the required quantity of water to form
divided into the following product groups: ready-to-use mortar based on the manufacturer’s
normal/finishing render or plaster, normal/finishing instructions and conditions. Delivered in sacks up to 35
render, or plaster with special properties, lightweight kg per sack or in silos up to 15 t per silo.
render, Reinforcement Fibre Plaster, and insulating
render with an especially high proportion of lightweight 2.5 Base materials/Ancillary materials
aggregates.
Placing normal/finishing render or plaster with special Mineral building products such as mineral pre-made
properties on the market in the EU/EFTA (with the mortars and rendering and plastering mortars mainly
exception of Switzerland) is subject to Regulation (EU) consist of abundant mineral raw materials. Scarcity of
No. 305/2011 (CPR). Normal/finishing render or plaster resources is not an issue.
with special properties requires a declaration of
performance – taking into consideration DIN EN 998-
1:2017-02, Specification for mortar for masonry - Part
1: Rendering and plastering mortar – and the CE Name Value Unit
marking. Aggregate 50-60 M.-%
The relevant national regulations apply with regard to Fine aggregate 15-20 M.-%
usage. Lightweight aggregate - M.-%
2.2 Application Artificial lightweight aggregate - M.-%
Rendering and plastering mortars produced in the Cement ≤ 15 M.-%
factory for use as a base coat or finishing Hydrated lime [Ca(OH2] ≤ 15 M.-%
render/plaster on walls, ceilings, piers, and separating
walls of structures which comply with the applicable The permissible fluctuation range of the constructional
standards or on similar backgrounds (e.g. in the case data is enabled by the variety of proportions of base
of existing buildings). materials. In each case, the composition of the
Normal render for the production of internal plaster and rendering and plastering mortars adds up to 100 m%.
external render with special properties (e.g. whiteness,
surface quality, or elasticity).
The following processing aids and admixtures can be
used as needed:
2.3 Technical Data
 Synthetic dispersion: < 2.50 m%
 Water retention agent: < 0.20 m%
Constructional data  Air entraining admixture: < 0.02 m%
 Thickening agent: < 0.03 m%
Name Value Unit
 Mineral pigments: < 0.50 m%
Compressive strength strength in
accordance with DIN EN 1015-11 ≤ 15 N/mm2  Hydrophobic agent: < 0.30 m%
Thermal conductivity in
accordance with DIN EN 1745 0.39 - 0.82 W/(mK) Aggregate: Natural sands as natural raw materials,
lambda10,dry,mat / P = 50 % which contain natural minor and trace minerals along
Thermal conductivity in with the main minerals quartz (SiO2) or calcite
accordance with DIN EN 1745 0,43 - 0,89 W/(mK) (CaCo3).
lambda10,dry,mat / P = 90 % Fine aggregate: Limestone dusts which arise as a
Sound absorption coefficient (as result of the preparation of natural sand for the
- %
required) production of aggregates, as well as ultra-fine sands.
Water-vapour transmission rate in Lightweight aggregate: Natural or artificial mineral
15/35 -
accordance with DIN EN 1015-19 lightweight aggregates for reducing the dry bulk
Dry bulk density in accordance 1300 - density. Natural lightweight aggregates are
kg/m³
with DIN EN 1015-10 1800 manufactured from natural raw materials via grinding
Capillary absorption in accordance kg/(m²min (e.g. pumice or vermiculite). Artificial lightweight
n/a
with DIN EN 1015-18 ^0,5) aggregates are manufactured by processing, melting,
and swelling suitable natural raw materials (swelling
clay, perlite) or sorted recycled glass (expanded
Performance values of normal/finishing render or glass).
plaster with special properties according to the Artificial lightweight aggregate: Organic, expanded
declaration of performance in relation to its key polystyrene (EPS) produced by foaming in spherical or
characteristics in accordance with DIN EN 998-1:2017- particle form (recycled) for reducing the dry bulk
02, Specification for mortar for masonry - Part 1: density.
Rendering and plastering mortar. Cement: As per DIN EN 197-1; cement is used as a
Adhesive shear strength, bond strength, and flexural binder and is mainly made from limestone marl or a
strength are not relevant. mixture of limestone and clay. The natural raw
materials are baked and then ground.
3 Environmental Product Declaration Sto SE & Co. KGaA – Mineral pre-made mortar: rendering and plastering mortar –
normal/finishing render or plaster with special properties
Hydrated lime: As per DIN EN 459; white hydrated
lime is used as a binder and is made by baking natural
limestone followed by slaking.
Synthetic dispersion: Polymer powder for improving
the adhesive bond, elasticity, mechanical properties,
etc. in thin-bed mortar.
Water retention agent: Cellulose ether, made from
cellulose, which prevents dehydration from occurring in
the fresh mortar too quickly.
Air entraining admixture: Surfactants for reducing
the surface tension of water and producing entrained
air. This reduces the bulk density of fresh mortar,
improves workability, and reduces the tendency
towards contraction and stress cracking.
Thickening agent: Cellulose or starch ether, made
from cellulose or crystal starch, improves the
resistance to flow, and thus has a thickening effect, but
does not have any water-retaining properties.
Mineral pigments: Natural or synthetic powder-form
Graphic 1: Manufacturing process (green: input; blue:
colouring materials which are produced by mechanical
unit process)
processing of the relevant mineral substances such as
chalk, clay, etc.
2.7 Environment and health during
Hydrophobic agent: Water-soluble sodium oleate or
manufacturing
zinc stearate for reducing the capillary absorption of
The current state of the art includes the 100 % return
the solid mortar.
of dry waste into production. In all places where dust
can arise during production in the factory, this waste is
Information about Substances of Very High Concern:
fed into a central filter system using the appropriate
The product contains substances from the ECHA
extraction systems, taking into account the
candidate list (15.01.2019) above 0.1 % w/w: no.
occupational limit values. The very fine dust filtered out
The product contains further CMR substances from
in these systems is then fed back into the
Category 1A or 1B which are not on the candidate list
manufacturing process. As part of the quality
above 0.1 % w/w in at least one part of the product: no.
management systems introduced, any off-specification
Biocide products have been added to this building
batches are detected immediately by the automated
product or it has been treated with biocide products
process monitoring system and are fed into circulation
(thus it is a treated product in the sense of the Biocide
via appropriate recovered-goods silos, i.e. they are fed
Products Ordinance (EU) No. 528/2012): no
back into the production process in very small
quantities. This procedure is also applied for product
2.6 Manufacture
residues which are transported back to the
The graphic shows the manufacturing process.
manufacturing plant in small quantities in silos or
Mineral rendering and plastering mortars are made in
sacks.
mixing plants in the following steps:
Process exhaust air is dedusted until the level is far
 Filling of the storage or weighing containers below the statutory occupational limit values.
 Conveyance of ingredients and substances
being mixed into the mixer Noise:
Noise level measurements have shown that all values
 Mixing
determined inside and outside the production facilities
 Conveyance of finished products
are well below the required specifications of the
 Packaging technical standards thanks to noise protection
 Loading and shipping of the finished product measures being taken.
2.8 Product processing/Installation
The raw materials – sand, binder, lightweight
Mineral rendering and plastering mortars are normally
aggregates, processing aids, admixtures, and
applied by machine. They are extracted from the silo
additions (see base materials) – are stored at the
with a dry-materials conveying machine or from
manufacturing plant in silos. From the silos, the raw
individual containers and mixed with a mixing pump
materials are gravimetrically dosed and intensely
before being conveyed and applied. Silo mixing pumps
mixed according to the respective formulation. The
can also be used.
mixture is then packaged and shipped dry as pre-made
The rendering and plastering mortars are then levelled,
dry mortar in containers or silos.
and textured if necessary, on site with suitable tools.
The regulations of the employers’ liability insurance
associations and the respective safety data sheets of
the building products apply.
With the cement and lime binders in mineral pre-made
mortars, the fresh mortar mixed with water is strongly
alkaline. Prolonged contact can cause serious skin
damage owing to the alkalinity. Personal protective
measures must therefore be taken (EU Health &
Safety Data Sheet) to avoid any contact with eyes or
skin.
4 Environmental Product Declaration Sto SE & Co. KGaA – Mineral pre-made mortar: rendering and plastering mortar –
normal/finishing render or plaster with special properties
No special measures are required for protection of the course.
environment. Unchecked dust emissions must be Normal/finishing render or plaster with special
avoided. properties is often used in external wall insulation
Mineral pre-made mortars must not enter the sewer systems which comply with the general building
system, surface water, or ground water. inspection requirements. The tests required in terms of
fire protection are always carried out on the entire
2.9 Packaging system. The reaction to fire of normal/finishing render
Bagged cargo from a paper bag with a plastic insert, or plaster with special properties is usually equivalent
sacks stored on wooden pallets, pallets wrapped in to or better than the approved system.
plastic film, silo-based goods stored in steel silos. Regardless of the product group, it has been shown in
Possibilities of reuse for the packaging of bagged the “hot” measurement (structural analysis with the
cargo – separation if necessary. Unsoiled polythene resistance of the masonry reduced under the influence
films (correct sorting must be applied) and reusable of fire temperatures) that rendering and plastering
wooden pallets are taken back by the building material mortar made from mineral pre-made mortars has a
dealer (reusable wooden pallets subject to beneficial effect on the required minimum wall
reimbursement as per the deposit system), returned to thickness.
the mortar plants by the dealer, and fed back into the Depending on the product, additional labels will appear
production process. The films are forwarded to the film on containers with the CE mark or declaration of
manufacturers for recycling. performance.
Fire protection
2.10 Condition of use Name Value
The specified products are rot-resistant and ageing- Building material class A1
resistant during normal use that conforms to the Burning droplets -
intended purpose of the products described. Smoke gas development -
Rendering and plastering mortars made from mineral
pre-made mortars must be protected from long-term Water
weather effects, e.g. by properly connecting the facade Mineral pre-made mortars as rendering and plastering
plinth (SAF). mortars are structurally stable and are not subject to
The cracking resistance of rendering and plastering changes in shape as a result of water exposure and
mortars made from mineral pre-made mortars can be drying.
increased with cracking reinforcement in the tension-
stressed areas of the render (DIN EN 13914-1, -2, DIN Mechanical destruction
18550-1, -2). No specifications required.
2.11 Environment and health during use 2.14 Re-use phase
Due to the stable calcium silicate hydrate (CSH) The service life of masonry coated with
adhesion and the firm structures achieved through normal/finishing render or plaster with special
curing on the substrate, emissions are rendered properties normally ends along with the service life of
impossible. During normal use conforming to the the simultaneously erected building. Reuse and further
intended purpose of the products described, any use of masonry coated with render after demolition is
adverse health effects have been rendered impossible. not possible.
No hazards for water, air, and soil are known for use Elements of building construction made from mineral
as per the intended application of the products. rendering and plastering mortars can normally be
The natural ionising radiation of the rendering and stripped down easily. During demolition of a building,
plastering mortars made from mineral pre-made these elements do not have to be treated as special
mortars is extremely low and does not pose any waste, but the sorting during demolition must be as
health-related risks. exact as possible. Mineral rendering and plastering
mortars can be recycled as building materials. They
2.12 Reference service life are normally reused in structural and civil engineering
A reference service life (RSL) as per ISO 15686-1, -2, - in the form of recycled aggregates.
7, and -8 is not declared. Provided they are used as
intended and properly applied, the service life of 2.15 Disposal
rendering and plastering mortars made from mineral Mortar is categorised as mineral construction waste.
pre-made mortars on walls and ceilings has been 78.4 % of construction waste is recycled. German
known to be 40 years or longer (BBSR). Building Materials Association
The suitability of hardened mineral rendering and
plastering mortars for landfill as per landfill class I is
2.13 Extraordinary effects ensured according to the Technical Instruction on
Municipal Waste (TASi). The EWC waste code
Fire according to the waste reuse directory is 170101.
Fire protection class A1
2.16 Further information
Because the proportion of finely dispersed organic Further information is available online at
components is greater than 1 %, the fire protection www.vdpm.info.
class A1 is always verified with a test as a matter of
3. LCA: Calculation rules
5 Environmental Product Declaration Sto SE & Co. KGaA – Mineral pre-made mortar: rendering and plastering mortar –
normal/finishing render or plaster with special properties
3.1 Declared Unit All of the background records relevant to the
This declaration refers to the production of one assessment have been retrieved from the GaBi8
kilogram of typical rendering and plastering mortar of database, with the exception of the pumice
the normal/finishing render or plaster product group (ROTOCELL) record.
with special properties. Only dry mortars are taken into
consideration. 3.6 Data quality
Representative products were used for this model EPD
Specification of declared unit – the product with the greatest environmental impact
was declared to be representative of a group in order
Name Value Unit to calculate the Life Cycle Assessment results.
Declared unit 1 kg Corresponding background records were available in
1300 - the GaBi database for all relevant primary products
Gross density kg/m3
1800 used.
Conversion factor to 1 kg 1 - The requirements in terms of data quality and
Spreading rate 0,70-0,85 l/kg background data correspond to the specifications of
PCR Part A.
The product which demonstrates the highest The technological background of the data collected
environmental impact of the normal/finishing render or reflects the physical reality for the declared product
plaster product group with special properties is group.
selected from that group for calculating the Life Cycle The records are complete and fulfil the system
Assessment. boundaries and criteria for the exclusion of inputs and
outputs.
The last audit of the data used was less than 8 years
3.2 System boundary ago.
The life cycle analysis of the products being examined
encompasses the production of the mortar including 3.7 Period under review
raw material extraction and the provision of energy The period under review is one year of production
sources up to the packaged, finished product (module based on the year 2018. The reference area of the Life
A1-A3), the application of the product including Cycle Assessments was limited to Germany. The
transportation to the construction site (module A4-A5), result is that, besides production processes under
the usage phase (module B1), and disposal of the these marginal conditions, the precursors also relevant
mortar (module C4). For silo-based goods, the for Germany, such as electricity and energy provision,
proportionate expenditure for transportation and were used.
manufacturing of the silo is taken into account. Credit
for packaging including energy recovery (module D) is 3.8 Allocation
also incorporated into the Life Cycle Assessment. Specific information on the allocations within the
background records can be found in the
3.3 Estimates and assumptions documentation of the GaBi records. The material and
For the individual formulation components of the energy consumption for the declared product were
formulations, these were assessed according to allocated by the member companies of the VDPM. The
manufacturer specifications or literature in the event data made available consists of internal key figures
that no specific GaBi 8 processes were available. which have not been published. A multi-input allocation
is used as per a simple credit method with a credit for
3.4 Cut-off criteria power and thermal energy when burning packaging
At the input side, all material flows that enter the and production waste as well as the landfilling of
system and are greater than 1 % of their total mass or production waste. The credit from the disposal of
contribute more than 1 % to primary energy demand packaging is credited in module D.
are taken into consideration. The total amount of input
flows not taken into consideration is maximum 5 % of 3.9 Comparability
the energy and mass in use. Basically, a comparison or an evaluation of EPD data
The manufacturing of the machines, facilities, and is only possible if all the data sets to be compared
other infrastructure required for the production of the were created according to EN 15804 and the building
relevant products was not taken into consideration for context, respectively the product-specific
the Life Cycle Assessments. characteristics of performance, are taken into account.
3.5 Background data The GaBi 8 background database was used for
The software system /GaBi8/ was used for modelling modelling purposes.
the life cycle for the production of the mortar products.
4. LCA: Scenarios and additional technical information
The following technical information is necessary for the Capacity utilisation (including
50 - 85 %
declared modules or can be used for the development empty runs)
of specific scenarios in the context of building Gross density of products 1300 -
kg/m3
assessment if modules have not been declared (MND). transported 1800
Transportation to the construction site (A4)
Name Value Unit Installation in the building (A5)
Litres of fuel 0.0062 l/100km Name Value Unit
Transport distance 300 km Auxiliary 0 kg
6 Environmental Product Declaration Sto SE & Co. KGaA – Mineral pre-made mortar: rendering and plastering mortar –
normal/finishing render or plaster with special properties
Water consumption 0.0003 m3
Other resources 0 kg
Electricity consumption 0.00045 kWh
Other energy carriers 0 MJ
Material loss 0 kg
Output substances following
0 kg
waste treatment on site
Dust in the air 0 kg
VOC in the air 0 kg
For use (B1) see Chapter 2.12 on use
In the use stage, the carbon dioxide absorbed by
means of carbonation is taken into consideration. The
carbon dioxide released during the neutralisation of
limestone (CaCO3) in the production of lime and
cement is reabsorbed when reacting with the lime and
cement binders, thus leading to an increase in
strength. In line with DIN EN 16757, the resulting
maximum theoretical carbon dioxide absorption for
fully carbonated rendering and plastering mortars and
the practical total maximum potential for carbon
dioxide absorption – taking into account the degree of
exposure of the surfaces – were calculated in the Life
Cycle Assessment of the pre-made mortar.
End of the life cycle (C1-C4)
Name Value Unit
Collected separately waste type 0 kg
Collected as mixed construction
0 kg
waste
Reuse 0 kg
Recycling 0 kg
Energy recovery 0 kg
Landfilling 1.06 kg
Reuse, recovery, and recycling potential (D);
relevant scenario specifications
Name Value Unit
Recycling silo (packaging) 100 %
Burning of wooden pallets
100 %
(packaging)
Burning of paper (packaging) 100 %
Burning of polythene film
100 %
(packaging)
7 Environmental Product Declaration Sto SE & Co. KGaA – Mineral pre-made mortar: rendering and plastering mortar –
normal/finishing render or plaster with special properties
5. LCA: Results
DESCRIPTION OF THE SYSTEM BOUNDARY (X = INCLUDED IN LCA; MND = MODULE NOT DECLARED;
MNR = MODULE NOT RELEVANT)
BENEFITS AND
CONSTRUCTI LOADS
PRODUCT STAGE ON PROCESS USE STAGE END OF LIFE STAGE BEYOND THE
STAGE SYSTEM
BOUNDARIES
8 Environmental Product Declaration Sto SE & Co. KGaA – Mineral pre-made mortar: rendering and plastering mortar –
normal/finishing render or plaster with special properties
lairetam
waR
ylppus tropsnarT
gnirutcafunaM
eht
morf
tropsnarT
etis
eht
ot
etag
ylbmessA esU
ecnanetniaM
riapeR
tnemecalpeR tnemhsibrufeR
ygrene
lanoitarepO esu
retaw
lanoitarepO esu
noitcurtsnoc-eD
noitilomed tropsnarT
gnissecorp
etsaW
lasopsiD -esueR -yrevoceR -gnilcyceR laitnetop
A1 A2 A3 A4 A5 B1 B2 B3 B4 B5 B6 B7 C1 C2 C3 C4 D
X X X X X X MND MNR MNR MNR MND MND MND MND MND X X
RESULTS OF THE LCA - ENVIRONMENTAL IMPACT according to EN 15804+A1: 1 kg Mineral pre-made
mortar: rendering and plastering mortar – normal/finishing render or plaster with special properties
Parameter Unit A1-A3 A4 A5 B1 C4 D
Global warming potential [kg CO2-Eq.] 3.74E-1 2.18E-2 4.17E-2 -1.62E-1 1.69E-2 -1.75E-2
Depletion potential of the stratospheric ozone layer [kg CFC11-Eq.] 2.49E-9 4.58E-16 5.71E-16 0.00E+0 3.76E-15 -1.27E-14
Acidification potential of land and water [kg SO2-Eq.] 9.20E-4 1.66E-5 5.46E-6 0.00E+0 9.99E-5 -1.91E-5
Eutrophication potential [kg (PO4)3--Eq.] 9.47E-5 3.74E-6 1.21E-6 0.00E+0 1.38E-5 -3.12E-6
Formation potential of tropospheric ozone photochemical
[kg ethene-Eq.] 7.67E-5 -2.35E-7 3.65E-7 0.00E+0 7.76E-6 -1.68E-6
oxidants
Abiotic depletion potential for non-fossil resources [kg Sb-Eq.] 8.61E-7 2.26E-9 7.30E-10 0.00E+0 6.49E-9 -4.04E-8
Abiotic depletion potential for fossil resources [MJ] 3.23E+0 2.92E-1 1.11E-2 0.00E+0 2.18E-1 -2.25E-1
RESULTS OF THE LCA - INDICATORS TO DESCRIBE RESOURCE USE according to EN 15804+A1: 1 kg
Mineral pre-made mortar: rendering and plastering mortar – normal/finishing render or plaster with
special properties
Parameter Unit A1-A3 A4 A5 B1 C4 D
Renewable primary energy as energy carrier [MJ] 4.96E-1 1.97E-2 2.88E-1 0.00E+0 2.81E-2 -5.23E-2
Renewable primary energy resources as material utilization [MJ] 2.86E-1 0.00E+0 -2.86E-1 0.00E+0 0.00E+0 0.00E+0
Total use of renewable primary energy resources [MJ] 7.82E-1 1.97E-2 2.37E-3 0.00E+0 2.81E-2 -5.23E-2
Non-renewable primary energy as energy carrier [MJ] 3.47E+0 2.93E-1 4.93E-2 0.00E+0 2.26E-1 -2.53E-1
Non-renewable primary energy as material utilization [MJ] 3.70E-2 0.00E+0 -3.70E-2 0.00E+0 0.00E+0 0.00E+0
Total use of non-renewable primary energy resources [MJ] 3.51E+0 2.93E-1 1.23E-2 0.00E+0 2.26E-1 -2.53E-1
Use of secondary material [kg] 0.00E+0 0.00E+0 0.00E+0 0.00E+0 0.00E+0 0.00E+0
Use of renewable secondary fuels [MJ] 0.00E+0 0.00E+0 0.00E+0 0.00E+0 0.00E+0 0.00E+0
Use of non-renewable secondary fuels [MJ] 0.00E+0 0.00E+0 0.00E+0 0.00E+0 0.00E+0 0.00E+0
Use of net fresh water [m³] 2.11E-2 2.29E-5 4.02E-4 0.00E+0 4.31E-5 -3.33E-5
RESULTS OF THE LCA – WASTE CATEGORIES AND OUTPUT FLOWS according to EN 15804+A1:
1 kg Mineral pre-made mortar: rendering and plastering mortar – normal/finishing render or plaster with
special properties
Parameter Unit A1-A3 A4 A5 B1 C4 D
Hazardous waste disposed [kg] 1.42E-8 1.88E-8 1.19E-11 0.00E+0 3.90E-9 -1.42E-10
Non-hazardous waste disposed [kg] 1.43E-2 2.18E-5 1.80E-4 0.00E+0 1.06E+0 -1.39E-4
Radioactive waste disposed [kg] 7.96E-5 3.54E-7 4.99E-7 0.00E+0 3.24E-6 -1.10E-5
Components for re-use [kg] 0.00E+0 0.00E+0 0.00E+0 0.00E+0 0.00E+0 0.00E+0
Materials for recycling [kg] 0.00E+0 0.00E+0 1.87E-4 0.00E+0 0.00E+0 0.00E+0
Materials for energy recovery [kg] 0.00E+0 0.00E+0 2.26E-2 0.00E+0 0.00E+0 0.00E+0
Exported electrical energy [MJ] 0.00E+0 0.00E+0 5.22E-2 0.00E+0 0.00E+0 0.00E+0
Exported thermal energy [MJ] 0.00E+0 0.00E+0 1.22E-1 0.00E+0 0.00E+0 0.00E+0
6. LCA: Interpretation
The LCA results are dominated by the life cycle environmental impact with a percentage of around 50 –
phases of raw material provision & transportation (A1 80 % – primarily due to the use of hydrated lime,
& A2), manufacture (particularly the manufacture of cement, dispersion powder, hydrophobic agent, and
packaging in A3), and landfill disposal (C4) in all pigments (together >80 % within A1). The manufacture
impact categories. Taken together, approx. 70 – 90 % of the dispersion powder dominates the indicator ODP
of the environmental impact comes from these life (>95 %). The indicator ADPE is dominated by the
cycle phases. hydrophobic agent (>60 %). Transportation of the raw
materials plays a secondary role (<10 % of total A1-
In total, raw materials used and their transportation A2).
contribute (excluding ODP and ADPE) to the
The manufacture of the packaging contributes (with the Landfill disposal at the end of the life cycle (C4)
exception of GWP, ODP, and PERT) approx. 5 – 15 %. contributes approx. 0 – 15 % to the environmental
The use of wooden pallets and paper contributes impact.
significantly to PERT (approx. 50 %).
In the usage phase, approx. 30 % of the GWP caused
Transportation of the products to the construction site is reabsorbed by means of carbonation (= carbon
(A4) plays a secondary role (<10 %). dioxide absorption).
7. Requisite evidence
7.1 Leaching:
All specified products in this LCA comply with all All specified products remained below the
emissions scenarios for a scenario involving the recommended limiting value.
building elements that are subject to moisture. 7.3 Radioactivity:
Measuring location: Fraunhofer Institute for Building
7.2 VOC emissions: Physics (IBP), Holzkirchen Branch, D-83626 Valley
Measuring location: Fraunhofer Institute for Building Measuring procedure: Test of content for the
Physics (IBP), Holzkirchen Branch, D-83626 Valley radioactive nuclides radium-226, thorium-232, and
Measuring procedure: Determination of volatile potassium-40 by measuring the activity concentrations
organic compounds from building products and fixtures CNuclide through alpha spectrometry (delayed
in accordance with DIN EN ISO 16000-9 and -11 in a coincidence method via LSC) or gamma spectrometry
0.2 m3 test chamber (t0 = 7 days) and evaluation as Test report: Inspection report from 12 December 2006
per the schema of the Committee for Health-related on the radioactivity of building products
Evaluation of Building Products (AgBB). Measurement Result: The activity concentration indices (I) calculated
of different products intended for both interior use and from the measured activity concentrations CNuclide
outdoors. were below the recommended limiting value of I = 2 for
Test report: Results log 005/2008/281 from 20 March all specified products. Moreover, at no point was the
2008 recommended limiting value I = 0.5 either reached or
Results: exceeded for building products used in large
quantities. Where I correlated with the dose criterion in
accordance with the Radiation Protection 112
guidelines from the European Commission, all
specified products remained below the recommended
limiting value of the annual radiation dose of 0.3
mSv/a.
8. References
PCR guidelines on building-related products and Core rules for the product category of construction
services, Part A: Calculation rules for the Life Cycle products.
Assessment and requirements on the project report,
Institut Bauen und Umwelt e. V., Version 1.7, 2018-03 GaBi 8
GaBi 8.7 dataset documentation for the software-
PCR guidelines on building-related products and system and databases, LBP, University of Stuttgart
services, Part B: Requirements on the EPD for and thinkstep, Leinfelden-Echterdingen, 2018
mineral pre-made mortars, Institut Bauen und Umwelt (http://documentation.gabi-software.com/)
e. V., Version 1.6, 2017-11
IBU 2016 DIN 4108-4
IBU (2016): General EPD programme instructions from DIN 4108-4:2017-03, Thermal insulation and energy
the economy in buildings - Part 4: Hygrothermal design
Institut Bauen und Umwelt e.V. (IBU). Version 1.1, values
Institut Bauen und Umwelt e.V., Berlin.
DIN 18550-1
ISO 14025 DIN 18550-1:2018-01, Design, preparation and
DIN EN ISO 14025:201110, application of external rendering and internal
Environmental labels and declarations - type III plastering - Part 1: Supplementary provisions for
environmental declarations - principles and DIN EN 13914-1:2016-09 for external rendering
procedures.
DIN 18550-2
EN 15804 DIN 18550-2:2018-01, Design, preparation and
EN 15804:201204+A1 2013, Sustainability of application of external rendering and internal
construction works - Environmental product plastering - Part 2: Supplementary provisions for
declarations - DIN EN 13914-2:2016-09 for internal plastering
9 Environmental Product Declaration Sto SE & Co. KGaA – Mineral pre-made mortar: rendering and plastering mortar –
normal/finishing render or plaster with special properties
DIN EN 13914-2 Corrigendum 1
DIN EN 197-1 DIN EN 13914-2 Corrigendum 1:2017-05, Design,
DIN EN 197-1:2011-11, Cement - Part 1: Composition, preparation and application of external rendering and
specifications, and conformity criteria for common internal plastering - Part 2: Internal plastering;
cements Corrigendum to DIN EN 13914-2:2016-09
DIN EN 450-1 DIN EN 16757
DIN EN 450-1:2012-10, Fly ash for concrete - Part 1: DIN EN 16757:2017-10, Sustainability of construction
Definition, specifications, and conformity criteria works - Environmental product declarations - Product
Category Rules for concrete and concrete elements
DIN EN 459-1
DIN EN 459-1:2015-07, Building lime - Part 1: DIN EN ISO 14040
Definitions, specifications, and conformity criteria DIN EN ISO 14040:2009-11, Environmental
management - Life cycle assessment - Principles and
DIN EN 998-1 framework (ISO 14040:2006)
DIN EN 998-1:2017-02, Specification for mortar for
masonry - Part 1: Rendering and plastering mortar DIN EN ISO 14044
DIN EN ISO 14044:2018-05, Environmental
DIN EN 1015-10 management - Life cycle assessment - Requirements
DIN EN 1015-10:2007-05, Methods of test for mortar and guidelines (ISO 14044:2006 + Amd 1:2017)
for masonry - Part 10: Determination of dry bulk
density of hardened mortar DIN EN ISO 16000-9
DIN EN ISO 16000-9:2008-04, Indoor air - Part 9:
DIN EN 1015-11 Determination of the emission of volatile organic
DIN EN 1015-11:2007-05, Methods of test for mortar compounds from building products and furnishing -
for masonry - Part 11: Determination of flexural and Emission test chamber method
compressive strength of hardened mortar
DIN EN ISO 16000-11
DIN EN 1015-18 DIN EN ISO 16000-11:2006-06, Indoor air - Part 11:
DIN EN 1015-18:2003-03, Methods of test for mortar Determination of the emission of volatile organic
for masonry - Part 18: Determination of water compounds from building products and furnishing -
absorption coefficient due to capillary action of Sampling, storage of samples and preparation of test
hardened mortar specimens
DIN EN 1015-19/ EC safety data sheet
DIN EN 1015-19:2005-01, Methods of test for mortar Available on the website of the relevant VDPM
for masonry - Part 19: Determination of water vapour member company.
permeability of hardened rendering and plastering
mortars ISO 15686-1
ISO 15686-1:2011-05, Buildings and constructed
DIN EN 1052-3 assets – Service life planning – Part 1: General
DIN EN 1052-3:2007-06, Methods of test for masonry - principles and framework
Part 3: Determination of initial shear strength
ISO 15686-2
DIN EN 1745 ISO 15686-2:2012-05, Buildings and constructed
DIN EN 1745:2012-07 Masonry and masonry products assets – Service life planning – Part 2: Service life
- Methods for determining thermal properties prediction procedures
DIN EN 12664 ISO 15686-7
DIN EN 12664: 2001-05, Thermal performance of ISO 15686-7:2017-04, Buildings and constructed
building materials and products - Determination of assets - Service life planning - Part 7: Performance
thermal resistance by means of guarded hot plate and evaluation for feedback of service life data from
heat flow meter methods - Dry and moist products with practice
medium and low thermal resistance
ISO 15686-8
DIN EN 13501-1 ISO 15686-8:2008-06, Buildings and constructed
DIN EN 13501-1:2010-01, Fire classification of assets - Service-life planning - Part 8: Reference
construction products and building elements - Part 1: service life and service-life estimation
Classification using data from reaction to fire tests
AgBB
DIN EN 13914-1 Committee for Health-related Evaluation of Building
DIN EN 13914-1:2016-09, Design, preparation and Products (AgBB): Procedure for the health-related
application of external rendering and internal plastering evaluation of volatile organic compound (VOC)
- Part 1: External rendering emissions from building products
DIN EN 13914-2 AVV
DIN EN 13914-2:2016-09, Design, preparation and Waste Catalogue Ordinance dated 10 December 2001
application of external rendering and internal plastering (Federal Law Gazette I p. 3379), last amended by
- Part 2: Internal plastering Article 2 of the Regulation of 17 July 2017 (Federal
Law Gazette I. p. 2644)
10 Environmental Product Declaration Sto SE & Co. KGaA – Mineral pre-made mortar: rendering and plastering mortar –
normal/finishing render or plaster with special properties
BBSR mixed dry render), January 2000 edition (unpublished)
BBSR - Federal Office for Building and Regional
Planning: Nutzungsdauern von Bauteilen für Commission Decision 94/611/EC
Lebenszyklusanalysen nach Bewertungssystem Commission Decision of 9 September 1994
Nachhaltiges Bauen (BNB) (Service lives of building implementing Article 20 of Directive 89/106/EEC on
elements for Life Cycle Assessments conducted construction products (94/611/EC)
according to the BNB Sustainable Building assessment
system), dated 24 February 2017 Life Cycle Assessment
Comparative Life Cycle Assessment: Masonry with
German Building Materials Association mineral mortar and masonry with PU foam bonding in
Bundesverband Baustoffe – Steine und Erden accordance with ISO 14040 and ISO 14044; carried
(German Building Materials Association) (Ed.): out on behalf of the VDPM (formerly IWM); Fraunhofer
Mineralische Bauabfälle – Monitoring 2010 (Mineral Institute for Building Physics IBP, Stuttgart/Holzkirchen
construction waste – monitoring 2010); Berlin, 2013 2008
DepV (2009) Radiation Protection 112
Ordinance on Landfills and Long-Term Storage European Commission: Radiation Protection 112
Facilities – Landfill Ordinance of 27 April 2009 (Federal “Radiological protection principles concerning the
Law Gazette I p. 900); last modified by Article 2 of the natural radioactivity of building materials”,
Regulation of 27 September 2017 (Federal Law Luxembourg: Publications Office of the European
Gazette I p. 3465). Union, 2000
ECHA candidate list SAF
European Chemicals Agency (ECHA): List of SAF – Fachverband der Stuckateure für Ausbau und
Substances of Very High Concern (published in Fassade Baden-Württemberg e.V. (Association of
accordance with Article 59 Para. 10 of the REACH Plasterers for Finishing and Facade) (Ed.): “Facade
Regulation) base render / outside facilities” guidelines, 3rd edition
2013
EWC waste code
Ordinance regarding the introduction of the European TASi
Waste Catalogue (EWC Ordinance) from 13 Technical Guidelines for the Recovery, Treatment and
September 1996: six-figure designation of types of Other Forms of Management of Domestic Waste (Third
waste, provided movable objects are waste according General Administrative Regulation for the Waste Act)
to Art. 3 Para. 1 of the Closed Substance Cycle and from 14 May 1993 (Federal Gazette No. 99a of 29 May
Waste Management Act 1993)
Industrieverband Werktrockenmörtel e.V. (WTM)
Internal study “Ökologische Aspekte von
Werktrockenmörtel” (Ecological aspects of ready
11 Environmental Product Declaration Sto SE & Co. KGaA – Mineral pre-made mortar: rendering and plastering mortar –
normal/finishing render or plaster with special properties
Publisher
Institut Bauen und Umwelt e.V. Tel +49 (0)30 3087748- 0
Panoramastr. 1 Fax +49 (0)30 3087748- 29
10178 Berlin Mail info@ibu-epd.com
Germany Web www.ibu-epd.com
Programme holder
Institut Bauen und Umwelt e.V. Tel +49 (0)30 - 3087748- 0
Panoramastr 1 Fax +49 (0)30 – 3087748 - 29
10178 Berlin Mail info@ibu-epd.com
Germany Web www.ibu-epd.com
Author of the Life Cycle
Assessment Tel +49 711 341817-0
thinkstep AG Fax +49 711 341817-25
Hauptstraße 111- 113 Mail info@thinkstep.com
70771 Leinfelden-Echterdingen Web http://www.thinkstep.com
Germany
Owner of the Declaration
Sto SE & Co. KGaA Tel +49 7744 57-1010
Ehrenbachstr. 1 Fax +49 7744 57-2010
79780 Stühlingen Mail infoservice@sto.com
Germany Web www.sto.com
