ENVIRONMENTAL PRODUCT DECLARATION
as per ISO 14025 and EN 15804+A2
Owner of the Declaration Grundfos Holding A/S
Publisher Institut Bauen und Umwelt e.V. (IBU)
Programme holder Institut Bauen und Umwelt e.V. (IBU)
Declaration number EPD-GRU-20240029-CBA1-EN
Issue date 20.03.2024
Valid to 19.03.2029
MIXIT 40-25 F
Grundfos Holding A/S
www.ibu-epd.com | https://epd-online.com
General Information
Grundfos Holding A/S MIXIT 40-25 F
Programme holder Owner of the declaration
IBU – Institut Bauen und Umwelt e.V. Grundfos Holding A/S
Hegelplatz 1 Poul Due Jensens Vej 7
10117 Berlin 8850 Bjerringbro
Germany Denmark
Declaration number Declared product / declared unit
EPD-GRU-20240029-CBA1-EN One piece of MIXIT 40-25 Flanged (F) control valve
This declaration is based on the product category rules: Scope:
control valves , 01.06.2023 The declared product is one piece of MIXIT 40-25 F control valve.
(PCR checked and approved by the SVR) This declaration covers all MIXIT Flanged (F) variants with the connection-
and flow combination 40-25.
Issue date The product is assembled in Germany.
The life cycle assessment is based on data collected from the ERP system
20.03.2024
of the manufacturer, including data from the production plant.
The owner of the declaration shall be liable for the underlying information
and evidence; the IBU shall not be liable with respect to manufacturer
Valid to
information, life cycle assessment data and evidences.
19.03.2029
The EPD was created according to the specifications of EN 15804+A2. In
the following, the standard will be simplified as EN 15804.
Verification
The standard EN 15804 serves as the core PCR
Independent verification of the declaration and data according to ISO
14025:2011
internally X externally
Dipl.-Ing. Hans Peters
(Chairman of Institut Bauen und Umwelt e.V.)
Florian Pronold Mrs Kim Allbury,
(Managing Director Institut Bauen und Umwelt e.V.) (Independent verifier)
1 Environmental Product Declaration - Grundfos Holding A/S - MIXIT 40-25 F
Product
Technically, a control valve is characterized by the following
Product description/Product definition
attributes, according to the PCR-B:
The declared product MIXIT is a prefabricated control valve unit
Control valve data
with integrated control functions. The unit integrates a
temperature controller, a balancing valve, an actuator, and Name Value Unit
temperature and flow sensors. Max valve capacity, Kvs 25 m3/h
This EPD covers MIXIT Flanged (F) variants with the
Nominal dimension of ports 40 (DN)
connection and flow size 40-25.
Nominal power input 8 W
For the placing on the market in the European Union/European Power input in stand-by mode 2.5 W
Free Trade Association (EU/EFTA) (with the exception of Number of ports 3 -
Switzerland) the following legal provisions apply: Liquid temperature range 0 - 90 °C
Ambient temperature range 0 - 50 °C
Machinery Directive (2006/42/EC)
Standards used: EN 60730-1:2016 + A1:2019, EN 60730-2- Performance data of the product according to the harmonised
8:2020, EN 60730-2-14:2019. standards, based on provisions for harmonization.
Base materials/Ancillary materials
Radio Equipment Directive (2014/53/EU)
Standards used: EN 60730-1:2016 + A1:2019, EN 60730-2- Main constituents of the product
8:2020, EN 60730-2-14:2019, EN 62479:2010, Name Value Unit
EN 61000-3-2:2019, EN 61000-3-3:2013 + A1:2019,
Cast iron and steel 69.2 %
ETSI EN 301 489-1 V2.2.3, ETSI EN 301 489-17 V3.2.3., ETSI
Stainless steel 4.7 %
EN 300 328 V2.2.2.
Brass 3.2 %
RoHS Directives (2011/65/EU and 2015/863/EU) Plastics incl. composites 7.3 %
Standards used: EN IEC 63000:2018. Plastic foam 1.2 %
Rubber 0.1 %
The CE-marking takes into account the proof of conformity with
Plastic film 0.0 %
the respective harmonized standards based on the legal
provisions above. Electronics 3.6 %
Paper 0.6 %
For the application and use the respective national provisions Corrugated board 10.1 %
apply.
"Plastics incl. composites" include thermoplastics and plastics
Application reinforced with glass fibres.
In a building application, a MIXIT unit is installed in series with a
REACH
water circulation pump to form a complete heating or cooling
The product does not contain substances listed in the
mixing loop. The matching circulation pump is not part of this
Candidate List of Substances of Very High Concern for
declaration. Mixing loops are used whenever there is a need for
Authorisation (August 2023) exceeding 0.1 percentage by
controlling (liquid) flow temperature. The basic principle is to
mass.
mix primary incoming water with return water to obtain the
required mixed flow temperature. MIXIT can be used in mixing
Reference service life
loops in heating and cooling systems where there is a need to
According to the PCR-B, a reference service life of 10 years
control water flow temperature, such as radiator heating,
has been assumed for the purpose of this study, for estimating
underfloor heating, air handling units, and cooling applications.
the energy consumption during the use stage of the control
Technical Data valve.
LCA: Calculation rules
materials extraction and processing, transportation, and the
Declared Unit manufacturing process. The product stage is included in this
The declared unit is one piece of MIXIT 40-25 Flanged (F) study, and according to EN 15804 the system boundary with
control valve. nature is set to include those processes that provide the
Declared unit and mass reference material and energy inputs into the system and the following
manufacturing, transport up to the factory gate as well as the
Name Value Unit
processing of waste arising from those processes. The
Declared unit 1 pce.
assembly of the product, as well as the packaging, are included
Mass reference 14.3 kg/pce in A3. Wastes and losses are included in the modules where
they occur according to the polluter pays principle and the
System boundary modular approach of EN 15804.
This EPD is classified as a Cradle-to-Grave and module D.
All major steps from the extraction of natural resources to the Module A4 regards the transportation from the production site
final disposal of the product are included in the scope of the to the regional distribution centre, and finally to the construction
study, following the modular approach of EN 15804. and product application site.
Module A5 refers to the installation process of the control valve,
Modules A1-A3 refer to the product stage and includes raw including the transportation of packaging waste to the treatment
2 Environmental Product Declaration - Grundfos Holding A/S - MIXIT 40-25 F
site and the waste treatment of packaging. The use of energy incineration. The End-of-Life assumption is that 95 % is
during installation is negligible for the selected functional unit. collected as electronic waste, while 5 % goes to landfill.
Modules B1-B7 refer to the use stage. All use stage modules Module D refers to the burdens and benefits beyond the system
are assessed in the study, though B1, B2 and B7 are assessed boundaries. According to EN 15804, module D includes the
to be zero. The modules B3, B4 and B5 are declared as reuse, recovery and/or recycling potentials, expressed in net
"MNR" (module not relevant) according to the PCR-B. impacts and benefits.
Module B6 regards energy use during the operation of the Contributions to module D come from waste incineration
product and includes the electricity consumption of the product. processes in A5 and C4 as well as material (metal) recycling in
The total electricity consumption over the reference service C3. The specific fractions and net flows are shown in the
lifetime is calculated by multiplying the power consumption in scenarios section.
activation and standby conditions, respectively, with the
reference values of annual activation and standby duration. The Geographic Representativeness
control valve is assumed to operate all year, with activation Land or region, in which the declared product system is
taking up 5 % of the total time. manufactured, used or handled at the end of the product´s
lifespan: Europe
Modules C1-C4 refer to the End-of-life stage. A product reaches
the end-of-life of its service life when it no longer provides any
Comparability
functionality. This life cycle stage includes all activities from the
Basically, a comparison or an evaluation of EPD data is only
end-of-life of the control valve until all materials and
possible if all the data sets to be compared were created
components are processed, reused, recycled, or disposed of.
according to EN 15804 and the building context, respectively
C1 regards the dismantling of the control valve, and this
the product-specific characteristics of performance, are taken
module is a manual activity. C2 regards the transport to waste
into account. The primary database used for background data
processing, C3 refers to the processing (shredding) of waste for
is Sphera, while Ecoinvent served as a secondary database.
recycling, and C4 refers to waste disposal: landfilling and
LCA: Scenarios and additional technical information
Operational energy use (B6) and Operational water use
Characteristic product properties of biogenic carbon
(B7)
In the declared net product, there is no biogenic carbon
exceeding the minimal reporting requirement of 5 % of the Name Value Unit
mass of the net product. Water consumption - m3
Note: 1 kg of biogenic carbon is equivalent to 44/12 kg of CO 2 Electricity consumption (Reference scenario) 243 kWh
Biogenic carbon content at factory gate The electricity consumption is calculated over the RSL for the
Name ValueUnit specified Usage conditions, and the power consumption at
activation and stand-by is specified in the Technical data table.
Biogenic carbon content in accompanying kg
0.62 The electricity mix applied for the reference scenario is a
packaging C
European residual mix, according to the PCR-B.
In the following, technical scenario information is provided for
End of life (C1-C4)
modules A4, A5, B6, C1-C4, and D.
Name ValueUnit
Collected separately waste type , Electronic waste
Transport from the gate to the site (A4) 12.8 kg
(WEEE)
Name Value Unit
Collected as mixed construction waste - kg
Transport distance 1500 km
Recycling ; Steel, incl. cast iron 9.4 kg
Capacity utilisation (including empty runs) 55 %
Recycling ; Stainless steel 0.6 kg
Gross density of products transported 331 kg/m3
Recycling ; Brass/Copper 0.4 kg
Assembly (A5) Incineration ; Plastics, electronics, paper 1.6 kg
Name Value Unit Landfilling 0.8 kg
Water consumption - m3
Reuse, recovery and/or recycling potentials (D), relevant
Electricity consumption - kWh scenario information
Packaging waste for incineration 1.44 kg Name ValueUnit
Reference lifetime: The PCR-B outlines a reference value of A5, Packaging incineration w/energy recovery ,
3.11 MJ
RSL as well as reference conditions of application to facilitate Electricity
reference building calculations: A Reference Service Life of 10 A5, Packaging incineration w/energy recovery ,
2.82 MJ
years is assumed together with running conditions fulltime, with Thermal energy
activation of the valve at 5 % of the time and standby conditions
C3, Copper for recycling , net output flow 0.008 kg
at 95 % of the time.
C3, Stainless steel for recycling , net output flow 0.57 kg
Reference service life
C4, Waste incineration w/energy recovery ,
5.90 MJ
Name Value Unit Electricity
Life Span according to the manufacturer 10 a C4, Waste incineration w/energy recovery , Thermal
5.30 MJ
Usage conditions: Operation time 100 % energy
Usage conditions: Activation fraction of operation 5 %
3 Environmental Product Declaration - Grundfos Holding A/S - MIXIT 40-25 F
LCA: Results
.
DESCRIPTION OF THE SYSTEM BOUNDARY (X = INCLUDED IN LCA; MND = MODULE OR INDICATOR NOT DECLARED; MNR
= MODULE NOT RELEVANT)
Benefits and
Construction loads beyond
Product stage Use stage End of life stage
process stage the system
boundaries
la ire ta m w a Ry lp p u s tro p s n a rT g n iru tc a fu n a M e h t m o rf tro p s n a rTe tis e h t o t e ta g y lb m e s s A e s U e c n a n e tn ia M ria p e R tn e m e c a lp e R tn e m h s ib ru fe R y g re n e la n o ita re p Oe s u re ta w la n o ita re p Oe s u n o itc u rts n o c -e Dn o itilo m e d tro p s n a rT g n is s e c o rp e ts a W la s o p s iD -e s u e R-y re v o c e R-g n ilc y c e Rla itn e to p
A1 A2 A3 A4 A5 B1 B2 B3 B4 B5 B6 B7 C1 C2 C3 C4 D
X X X X X X X MNR MNR MNR X X X X X X X
RESULTS OF THE LCA - ENVIRONMENTAL IMPACT according to EN 15804+A2:
Parameter Unit A1 A2 A3 A4 A5 B1 B2 B6 B7 C1 C2 C3 C4 D
-1.02E
GWP-total kg CO 2 eq 5.38E+01 1.03E+00 +00 2.07E+00 2.06E+00 0 0 1.01E+02 0 0 5.46E-01 3.01E-01 3.4E+00 -3.49E+00
GWP-fossil kg CO 2 eq 5.33E+01 1.03E+00 1.24E+00 2.08E+00 7.05E-02 0 0 1.01E+02 0 0 5.49E-01 3.02E-01 3.29E+00-3.48E+00
GWP- -2.27E
biogenic kg CO 2 eq 4.46E-01 -1.02E-02 +00 -3.06E-02 1.99E+00 0 0 3.94E-02 0 0 -8.07E-03 -8.42E-04 1.08E-01 -1.26E-02
GWP-luluc kg CO 2 eq 3.78E-02 6.78E-03 5.85E-03 1.92E-02 1.41E-04 0 0 9.38E-03 0 0 5.07E-03 9.61E-05 4.74E-05 -3.98E-04
kg CFC11
ODP 3.87E-08 1.04E-13 3.16E-12 2.7E-13 2.52E-13 0 0 1.01E-09 0 0 7.12E-14 6.9E-10 3.79E-13 -1.5E-11
eq
AP mol H+ eq 1.28E-01 7.31E-03 4.01E-03 3.76E-03 5.88E-04 0 0 1.56E-01 0 0 9.93E-04 1.16E-03 8.98E-04 -2.08E-02
EP-
kg P eq 5.3E-04 2.73E-06 3.72E-05 7.59E-06 1.29E-07 0 0 1.01E-04 0 0 2E-06 3.74E-05 3E-06 -4.92E-06
freshwater
EP-marine kg N eq 3.06E-02 3.06E-03 1.9E-03 1.51E-03 2.15E-04 0 0 4.4E-02 0 0 3.99E-04 2.02E-04 3.45E-04 -2.88E-03
EP-terrestrial mol N eq 2.86E-01 3.38E-02 1.86E-02 1.73E-02 2.68E-03 0 0 4.65E-01 0 0 4.56E-03 2.52E-03 4.39E-03 -3.1E-02
kg
POCP NMVOC 7.85E-02 8.08E-03 4.65E-03 3.37E-03 5.65E-04 0 0 1.22E-01 0 0 8.9E-04 5.94E-04 9.24E-04 -8.97E-03
eq
ADPE kg Sb eq 9.96E-04 5.1E-08 4.57E-07 1.38E-07 3.2E-09 0 0 4.97E-06 0 0 3.63E-08 5.13E-06 2.86E-09 -1.23E-04
ADPF MJ 7.65E+02 1.38E+01 1.84E+01 2.83E+01 8.34E-01 0 0 2.25E+03 0 0 7.46E+00 5.97E+00 1.36E+00-4.81E+01
m3 world
WDP eq 2.84E+00 9.04E-03 1.22E-01 2.51E-02 2.54E-01 0 0 8.62E+00 0 0 6.62E-03 7.38E-02 3.42E-01 -2.88E-01
deprived
GWP = Global warming potential; ODP = Depletion potential of the stratospheric ozone layer; AP = Acidification potential of land and water; EP =
Eutrophication potential; POCP = Formation potential of tropospheric ozone photochemical oxidants; ADPE = Abiotic depletion potential for non-fossil
resources; ADPF = Abiotic depletion potential for fossil resources; WDP = Water (user) deprivation potential)
RESULTS OF THE LCA - INDICATORS TO DESCRIBE RESOURCE USE according to EN 15804+A2:
Parameter Unit A1 A2 A3 A4 A5 B1 B2 B6 B7 C1 C2 C3 C4 D
PERE MJ 3E+02 7.31E-01 1.26E+01 2.06E+00 2.18E+01 0 0 3.09E+02 0 0 5.43E-01 3.4E+00 1.42E+00 -1.02E+01
-1.18E
PERM MJ 1.18E+00 0 2.16E+01 0 -2.16E+01 0 0 0 0 0 0 0 0
+00
PERT MJ 3.01E+02 7.31E-01 3.42E+01 2.06E+00 1.7E-01 0 0 3.09E+02 0 0 5.43E-01 3.4E+00 2.41E-01 -1.02E+01
PENRE MJ 7.29E+02 1.38E+01 1.83E+01 2.84E+01 9.64E-01 0 0 2.25E+03 0 0 7.49E+00 5.97E+00 3.49E+01 -4.81E+01
-3.35E
PENRM MJ 3.63E+01 0 1.29E-01 0 -1.29E-01 0 0 0 0 0 0 0 0
+01
PENRT MJ 7.65E+02 1.38E+01 1.84E+01 2.84E+01 8.35E-01 0 0 2.25E+03 0 0 7.49E+00 5.97E+00 1.36E+00 -4.81E+01
SM kg 1.04E+01 0 1.28E+00 0 0 0 0 0 0 0 0 0 0 0
RSF MJ 0 0 0 0 0 0 0 0 0 0 0 0 0 0
NRSF MJ 0 0 0 0 0 0 0 0 0 0 0 0 0 0
FW m3 1.89E-01 8.06E-04 1.7E-02 2.25E-03 5.99E-03 0 0 5.16E-01 0 0 5.95E-04 3E-03 8.04E-03 -1.03E-02
PERE = Use of renewable primary energy excluding renewable primary energy resources used as raw materials; PERM = Use of renewable primary
energy resources used as raw materials; PERT = Total use of renewable primary energy resources; PENRE = Use of non-renewable primary energy
excluding non-renewable primary energy resources used as raw materials; PENRM = Use of non-renewable primary energy resources used as raw
materials; PENRT = Total use of non-renewable primary energy resources; SM = Use of secondary material; RSF = Use of renewable secondary fuels;
NRSF = Use of non-renewable secondary fuels; FW = Use of net fresh water
RESULTS OF THE LCA – WASTE CATEGORIES AND OUTPUT FLOWS according to EN 15804+A2:
Parameter Unit A1 A2 A3 A4 A5 B1 B2 B6 B7 C1 C2 C3 C4 D
HWD kg 1.12E-04 3.45E-11 4.41E-07 8.78E-11 2.1E-11 0 0 1.31E-07 0 0 2.32E-11 6.85E-10 7.71E-11 -3.98E-04
NHWD kg 1.32E+00 2.13E-03 5.08E-02 4.32E-03 6.42E-02 0 0 4.97E-01 0 0 1.14E-03 3.98E-03 9.07E-01 8.91E-02
RWD kg 3.38E-02 2E-05 5.48E-04 5.31E-05 3.46E-05 0 0 3.51E-01 0 0 1.4E-05 8.63E-04 4.65E-05 -2.91E-03
CRU kg 0 0 0 0 0 0 0 0 0 0 0 0 0 0
4 Environmental Product Declaration - Grundfos Holding A/S - MIXIT 40-25 F
MFR kg 0 0 0 0 0 0 0 0 0 0 0 1.05E+01 0 0
MER kg 0 0 0 0 0 0 0 0 0 0 0 0 0 0
EEE MJ 0 0 0 0 3.11E+00 0 0 0 0 0 0 0 5.9E+00 0
EET MJ 1.08E-01 0 7.13E-04 0 2.82E+00 0 0 0 0 0 0 0 5.3E+00 0
HWD = Hazardous waste disposed; NHWD = Non-hazardous waste disposed; RWD = Radioactive waste disposed; CRU = Components for re-use;
MFR = Materials for recycling; MER = Materials for energy recovery; EEE = Exported electrical energy; EET = Exported thermal energy
RESULTS OF THE LCA – additional impact categories according to EN 15804+A2-optional:
Parameter Unit A1 A2 A3 A4 A5 B1 B2 B6 B7 C1 C2 C3 C4 D
Disease
PM 2.17E-06 1.75E-07 7.03E-08 4.64E-08 3.39E-09 0 0 1.41E-06 0 0 1.23E-08 9.91E-09 6.14E-09 -4.77E-07
incidence
kBq U235
IR 3.74E+00 2.91E-03 9.06E-02 7.92E-03 5.48E-03 0 0 5.27E+01 0 0 2.09E-03 1.45E-01 7.24E-03 -4.7E-01
eq
ETP-fw CTUe 4.08E+02 1.04E+01 4.61E+00 2.02E+01 4.05E-01 0 0 1.96E+02 0 0 5.34E+00 2.35E+00 6.9E-01 -7.87E+00
HTP-c CTUh 1.18E-06 2.08E-10 2.66E-10 4.11E-10 1.96E-11 0 0 1.16E-08 0 0 1.08E-10 3.63E-10 6.29E-11 -8.81E-08
HTP-nc CTUh 4.66E-07 8.9E-09 1.24E-08 1.83E-08 5.36E-10 0 0 3.74E-07 0 0 4.82E-09 1.79E-08 3.69E-09 -2.05E-08
SQP SQP 2.62E+02 4.17E+00 7.79E+01 1.18E+01 2.67E-01 0 0 3.05E+02 0 0 3.12E+00 3.5E+00 2.73E-01 -6.98E+00
PM = Potential incidence of disease due to PM emissions; IR = Potential Human exposure efficiency relative to U235; ETP-fw = Potential comparative
Toxic Unit for ecosystems; HTP-c = Potential comparative Toxic Unit for humans (cancerogenic); HTP-nc = Potential comparative Toxic Unit for humans
(not cancerogenic); SQP = Potential soil quality index
Disclaimer 1 – for the indicator 'Potential Human exposure efficiency relative to U235'. This impact category deals mainly with the
eventual impact of low-dose ionizing radiation on human health of the nuclear fuel cycle. It does not consider effects due to possible
nuclear accidents, occupational exposure or radioactive waste disposal in underground facilities. Potential ionizing radiation from the
soil, radon and from some construction materials is also not measured by this indicator.
Disclaimer 2 – for the indicators 'abiotic depletion potential for non-fossil resources', 'abiotic depletion potential for fossil resources',
'water (user) deprivation potential, deprivation-weighted water consumption', 'potential comparative toxic unit for ecosystems', 'potential
comparative toxic unit for humans – cancerogenic', 'Potential comparative toxic unit for humans - not cancerogenic', 'potential soil
quality index'. The results of this environmental impact indicator shall be used with care as the uncertainties on these results are high
as there is limited experience with the indicator.
The module B6 has been calculated for a Reference Service Life of 10 years.
References
ETSI EN 300 328 Wideband transmission systems; Data
Candidate List of substances of very high concern for transmission equipment operating in the 2,4 GHz band;
Authorisation (published in accordance with Article 59(10) of Harmonised Standard for access to radio spectrum
the REACH Regulation). Available at
https://echa.europa.eu/candidate-list-table Machinery Directive 2006/42/EC
Directive 2006/42/EC of the European Parliament and of the
EN 15804 Council of 17 May 2006 on machinery, and amending Directive
EN 15804:2012+A2:2019+AC:2021, Sustainability of 95/16/EC
construction works — Environmental Product Declarations —
Core rules for the product category of construction products. Radio Equipment Directive (2014/53/EU)
Directive 2014/53/EU of the European Parliament and of the
ISO 14025 Council of 16 April 2014 on the harmonisation of the laws of the
EN ISO 14025:2011, Environmental labels and declarations — Member States relating to the making available on the market
Type III environmental declarations — Principles and of radio equipment and repealing Directive 1999/5/EC
procedures.
RoHS Directives (2011/65/EU) and (2015/863/EU)
EN 60730 Automatic electrical controls. Part 1: General EN IEC 63000:2018 Technical documentation for the
requirements. Part 2: Particular requirements. assessment of electrical and electronic products with respect to
the restriction of hazardous substances.
EN IEC 61000 Electromagnetic compatibility (EMC). Part 3-2:
Limits - Limits for harmonic current emissions. Part 3-3: Limits – IBU 2022
Limitation of voltage changes, voltage fluctuations and flicker in Institut Bauen und Umwelt e.V.: General Instructions for the
public low-voltage supply systems EPD programme of Institut Bauen und Umwelt e.V., Version
2.1, Berlin: Institut Bauen und Umwelt e.V., 2022, www.ibu-
EN IEC 62479:2010 Assessment of the compliance of low- epd.com
power electronic and electrical equipment with the basic
restrictions related to human exposure to electromagnetic fields Software and database
(10 MHz to 300 GHz) Sphera LCA for Experts, v. 10.7.1.28,
incl. Sphera Professional Database v. 2023.1
EN IEC 63000:2018 Technical documentation for the Additional database: Ecoinvent v. 3.9.1
assessment of electrical and electronic products with respect to
the restriction of hazardous substances
PCR-A
ETSI EN 301 489 ElectroMagnetic Compatibility (EMC) Product Category Rules for Building-Related Products and
standard for radio equipment and services Services, Part A: Calculation Rules for the Life Cycle
Assessment and Requirements on the Project Report according
5 Environmental Product Declaration - Grundfos Holding A/S - MIXIT 40-25 F
to EN 15804+A2:2019. Version 1.3, 2021. PCR Guidance-Text for Building-Related Products and
Services, Part B: Requirements on the EPD for control valves.
PCR-B Version 1, 2023.
6 Environmental Product Declaration - Grundfos Holding A/S - MIXIT 40-25 F
Publisher
Institut Bauen und Umwelt e.V. +49 (0)30 3087748- 0
Hegelplatz 1 info@ibu-epd.com
10117 Berlin www.ibu-epd.com
Germany
Programme holder
Institut Bauen und Umwelt e.V. +49 (0)30 3087748- 0
Hegelplatz 1 info@ibu-epd.com
10117 Berlin www.ibu-epd.com
Germany
Author of the Life Cycle Assessment
Grundfos Holding A/S +4587501400
Poul Due Jensens Vej 7 LCA_EPD@grundfos.com
8850 Bjerringbro www.grundfos.com
Denmark
Owner of the Declaration
Grundfos Holding A/S +4587501400
Poul Due Jensens Vej 7 LCA_EPD@grundfos.com
8850 Bjerringbro www.grundfos.com
Denmark
7 Environmental Product Declaration - Grundfos Holding A/S - MIXIT 40-25 F
