ENVIRONMENTAL PRODUCT DECLARATION
as per ISO 14025 and EN 15804+A2
Owner of the Declaration Etex Building Performance International
Publisher Institut Bauen und Umwelt e.V. (IBU)
Programme holder Institut Bauen und Umwelt e.V. (IBU)
Declaration number EPD-ETE-20230251-IBA1-EN
Issue date 25/09/2023
Valid to 24/09/2028
Monalite® M1AT and Monalite® M1T
PROMAT
www.ibu-epd.com | https://epd-online.com
1. General Information
PROMAT Monalite® M1AT and Monalite® M1T
Programme holder Owner of the declaration
IBU – Institut Bauen und Umwelt e.V. Etex Building Performance International
Hegelplatz 1 Rue Marcel Demonque 500
10117 Berlin 84915 Avignon Cedex 9
Germany France
Declaration number Declared product / declared unit
EPD-ETE-20230251-IBA1-EN 1 m2 of Monalite® M1AT/Monalite® M1T with a thickness of 38.5 mm
This declaration is based on the product category rules: Scope:
Calcium silicate insulating materials, 01/08/2021 This EPD is representative and relevant for Monalite® M1AT/Monalite®
(PCR checked and approved by the SVR) M1T boards produced by ETEX in Tisselt (Belgium) and installed in
Europe. The data describing the direct inputs and outputs of the
foreground processes are representative for ETEX production in Tisselt,
Issue date Belgium, and taken from the period of one year between October 2020
and September 2021.
25/09/2023
The results in this EPD are based on Monalite® M1AT. In the LCA
background report, the representativeness of Monalite® M1AT has been
Valid to
checked by comparing the results of Monalite® M1AT and Monalite® M1T.
24/09/2028 This study showed that for all environmental impact indicators Monalite®
M1AT is the most conservative product, and as a result representative for
the product range included in the EPD.
The owner of the declaration shall be liable for the underlying information
and evidence; the IBU shall not be liable with respect to manufacturer
information, life cycle assessment data and evidences.
The EPD was created according to the specifications of EN 15804+A2. In
the following, the standard will be simplified as EN 15804.
Verification
The standard EN 15804 serves as the core PCR
Dipl.-Ing. Hans Peters
Independent verification of the declaration and data according to ISO
(Chairman of Institut Bauen und Umwelt e.V.)
14025:2011
internally X externally
Florian Pronold Vito D'Incognito,
(Managing Director Institut Bauen und Umwelt e.V.) (Independent verifier)
1 Environmental Product Declaration - PROMAT - Monalite® M1AT and Monalite® M1T
2. Product
Name Value Unit
2.1 Product description/Product definition
Gross density EN12467 850 - 992 kg/m3
Monalite® M1AT and Monalite® M1T
This EPD describes the life cycle analysis of two Promat Compressive strength EN 993-5 2000 <21 N/mm2
products for fire protection in heavy industries. The products (cold)
under consideration are the cement-bounded high-density Flexural strength EN 993-6 1995 >8.0 N/mm2
calcium silicate fire protective boards. In detail the investigated 0.274 -
products are 2 for this group including Monalite® M1AT and Thermal conductivity at 200°C 0.299 W/(mK)
Monalite® M1A. The results in this EPD are based on
0.283 -
Monalite® M1AT. In the LCA background report, the Thermal conductivity at 500°C W/(mK)
0.297
representativeness of Monalite® M1AT has been checked by
0.294 -
comparing the LCA results of Monalite® M1AT and Monalite® Thermal conductivity at 800°C W/(mK)
0.303
M1T. This study showed that for all environmental impact
indicators Monalite® M1AT is the most conservative product,
and as a result representative for the product range included in Product for which no legal provisions for harmonisation of the
the EPD. EU exist. For the use and application of the product the
respective national provisions at the place of use apply.
Monalite® materials are asbestos-free made from calcium
silicate. These boards are used in aluminum casting and the 2.4 Delivery status
foundry industry and are also used in the furnace industry and The products have a thickness of 13.1, 19.5, 25.8, 38.5, 51.2,
other process industries. The products differentiate by 76.6 or 102 mm.
individual densities and the ratios of included raw materials to The length is 2500 mm.
meet the technical requirements of individual applications with The width is 1200 mm.
direct contact to molten metals up to 1000°C. Monalite is the
only non-wettable product in the Promat range. The products are transported and delivered on a wooden pallet
Product for which no legal provisions for harmonisation of the and packed with cartons and PET straps.
EU exist. For the use and application of the product the
2.5 Base materials/Ancillary materials
respective national provisions at the place of use apply.
The main constituents of the product are silica (10-25 %),
2.2 Application wollastonite (40-60 %), cement (1-10 %), lime (10-20 %) and
Monalite® M1AT and Monalite® M1T boards are versatile multi- cellulose fibres (1-10 %).
purpose fire protection boards, for multiple applications:
This product/article/at least one partial article contains
Oil and gas substances listed in the candidate list (date: accesses
31/07/2023) exceeding 0.1 percentage by mass: no
• Collars, gaskets and pipe support rings
• Spacers and bushes
This product/article/at least one partial article contains other
• Thermal separation for high loads
carcinogenic, mutagenic, reprotoxic (CMR) substances in
Heavy industry
categories 1A or 1B which are not on the candidate list,
• The non wetting properties of Monalite mean that these exceeding 0.1 percentage by mass: no
products are ideally suited for use in non-ferrous casting
applications Biocide products were added to this construction product or it
• Billet and ingot casting as transition plates, floats, has been treated with biocide products (this then concerns a
spouts treated product as defined by the (EU) Ordinance on Biocide
• Head boxes for continuous casters Products No. 528/2012): no
• Tips for continuous sheet casters
• Sprue bushes, tubes, nozzles and feeder box liner in 2.6 Manufacture
low pressure die casting There is only one manufacturing plant of the declared products
• Hotfacelinings for dosing/holding furnaces being the manufacturing plant in Tisselt (Belgium). The
• Launders and dams products are all produced on the same type of production line.
• Load bearing housings All raw materials, including previously made xonotlite slurries,
• Structural insulation where high thermal and/or together with a balanced amount of water are mixed to form a
mechanical load is required slurry, and shaped by a filter press to produce a wet board. It is
steam cured in an autoclave to form required calcium silicate
2.3 Technical Data
minerals suitable for the end application. Final steps are the
Constructional data drying, cutting and sanding/finishing. During the cutting and
finishing, scrap is produced which is partly recycled, both
internally and externally, and partly landfilled.
2.7 Environment and health during manufacturing
Environmental, occupational health, safety and quality
management at the Guangzhou plant are in accordance with
the following standards:
· ISO 14001;2015
· ISO 9001;2015
· ISO 45001:2018
2.8 Product processing/Installation
2 Environmental Product Declaration - PROMAT - Monalite® M1AT and Monalite® M1T
Not considered in the EPDs. Various installation scenarios exist Name Value
depending on the application. Building material class A1
Burning droplets /
2.9 Packaging
The products are transported and delivered on a wooden pallet Smoke gas development /
and packed with cartons and PET straps.
Water
2.10 Condition of use
Tests on the product performance including possible impacts on
B modules are not included. These products are designed for
the environment following the unforeseeable influence of water,
life and depending on the application in which the products are
e.g. flooding showed that no risks are expected to occur in
used there might be a need for
terms of environment and human health.
maintenance/repair/replacement of the application.
Mechanical destruction
2.11 Environment and health during use
In case of mechanical destruction, no risks are expected to
Under normal conditions of use, the products do not cause any
occur in terms of environment and human health.
adverse health effects or release of volatile organic compounds
(VOCs) into indoor air. No environmental impact on water, air or 2.14 Re-use phase
soil is expected due to the extremely low metal release from the
Currently, the boards can be recycled as a replacement of filler
low maintenance requirements.
(e.g. secondary limestone fillers). In the EPD, both the 100 %
recycling and 100 % landfill scenario have been calculated.
2.12 Reference service life
The RSL depends on the application. Under normal conditions 2.15 Disposal
of use, the product is supposed to remain its characteristics as
The waste number according to the European list 'Decision N°
long as the application lasts. For application in building a
2000/532/CE' is '17 09 00: other construction and demolition
reference service life of 60 years (i.e life time of the building)
wastes'.
could be declared.
2.16 Further information
2.13 Extraordinary effects
https://www.promat.com/en/industry/products-solutions/high-
Fire
temperature-insulation/boards-hti/monalite/
Information on the fire performance according to EN 13501:1.
Fire protection
3. LCA: Calculation rules
3.1 Declared Unit 3.3 Estimates and assumptions
1 m2 of Monalite® M1AT/Monalite® M1T with a thickness of The results in this EPD are based on Monalite® M1AT. In the
38.5 mm LCA background report the representativeness of Monalite®
M1AT has been checked by comparing the LCA results of
Declared unit
Monalite® M1AT and Monalite® M1T. This study showed that
Name Value Unit for all environmental impact indicators Monalite® M1AT is the
Declared unit 1 m² most conservative product, and as a result representative for
Gross density 992 kg/m3 the product range included in the EPD.
Grammage 38.19 kg/m2 3.4 Cut-off criteria
Conversion factor to 1 kg 0.026 The following processes are considered below cut-off according
Layer thickness 0.0385 m to the rules as per the PCR, Part A:
The results in this EPD are based on Monalite® M1AT. In the • Packaging of raw materials, as the main raw materials
LCA background report the representativeness of Monalite® (i.e. largest amounts) come in bulk.
M1AT has been checked by comparing the LCA results of • Ancillary materials for production
Monalite® M1AT and Monalite® M1T. • Infrastructure and land use of the factory
• Environmental impacts caused by the
Assuming a linear relationship between the thickness and the personnel of the production plants are not included in
mass/environmental impact of the board, the environmental the LCA, e.g. waste from
impact of a product can be considered to be proportional to the the cafeteria and sanitary installations, accidental
thickness of the product, so products with another thickness pollution caused by human
can be calculated by the below formula: mistakes, or environmental effects caused by commuter
traffic. Heating or
E=W*Eref/Wref cooling of the plants in order to ensure a comfortable
indoor climate for the
E=environmental impact of a product with density d and personnel for example is also neglected.
thickness t
3.5 Background data
W=d*t=weight of 1 m2 product with density d and thickness t
Ecoinvent 3.8 and Industry 2.0
Eref=environmental impact of the reference product
Wref=weight of 1 m2 reference product 3.6 Data quality
Company-specific data concern the data about the production
of Monalite® M1AT. All required data about the production
3.2 System boundary process have been delivered to Enperas by ETEX.
Cradle-to-gate with options, including modules C2-C4 and D
3 Environmental Product Declaration - PROMAT - Monalite® M1AT and Monalite® M1T
The composed datasets for this project are representative and product in m2.5 (i.e. 1 m2 with a thickness of 5 mm is the
relevant for Monalite® M1AT and Monalite® M1T produced by reference unit in ETEX's factory). The last step was to
ETEX in Tisselt, Belgium. recalculate the amount to the declared unit by multiplying with
the mass ratio between 1 m2.5 and 1 m2 with the thickness
3.7 Period under review
declared in the EPD. This approach has been used for all
The data collected by ETEX are based on data from the period
inputs and outputs, except for water use/discharge and
of one year between October 2020 and September 2021.
production waste-externally recycled.
For the water use/discharge only facility-level data were
3.8 Geographic Representativeness
available. These have been allocated to the individual product
Land or region, in which the declared product system is
using the annual production volume in kg. For the production
manufactured, used or handled at the end of the product´s
waste-externally recycled, facility-level data were available for
lifespan: Europe
all the declared products together with two other Promat
products of the Tisselt plant. These have been allocated to the
3.9 Allocation individual product using the annual production volume in kg.
No co-products are produced.
No secondary raw materials are used. 3.10 Comparability
At ETEX's plant in Tisselt, different types of calcium silicate Basically, a comparison or an evaluation of EPD data is only
boards are produced. possible if all the data sets to be compared were created
For most of the production data, product specific data is according to EN 15804 and the building context, respectively
available, as the data per production step or product line could the product-specific characteristics of performance, are taken
be extracted. In this case, the data have been allocated to the into account. Ecoinvent 3.8 and Industry 2.0
declared unit using the annual production volume of that
4. LCA: Scenarios and additional technical information
3. the remaining powder (<100µm) will be used as a filler
Characteristic product properties of biogenic carbon replacing limestone in concrete applications or fibre
The Promat boards contain biogenic carbon in the form of cement production.
cellulose (assumed 0,44 kg C/kg cellulose). Also, its packaging Name ValueUnit
contains biogenic carbon in the form of cartons (assumed 0,44
Collected as mixed construction waste 38.19 kg
kg C/kg carton) and wooden pallets (assumed 0,45 kg C/kg
Recycling Scenario 1 (cellulose content is
wood). 38.19 kg
incinerated)
Information on describing the biogenic carbon content at
Landfilling Scenario 2 38.19 kg
factory gate
Reuse, recovery and/or recycling potentials (D), relevant
Name ValueUnit
scenario information
kg
Biogenic carbon content in product 0.679 In module D, the benefits and loads beyond the system
C
boundaries are quantified. For recycling, it concerns both the
Biogenic carbon content in accompanying 0.402 kg loads of the recycling processes after the end-of-waste and the
packaging C benefits of the avoided virgin materials, when the recycled
components are used for other purposes. In case of
incineration, it concerns the benefits from the avoided
production of energy grace to energy recovery.
End of life (C1-C4)
In the EPD, both 100 % recycling and 100 % landfill scenario
Benefits of recycling the product in limestone production have
have been calculated. Recycling consists in
been included in module D (avoided impact of limestone
1. milling/crushing the boards production and energy recovery from incineration of cellulose),
2. sieving out the fibres which will be incinerated and used together with some minor benefits and loads due to recycling
as an energy source (to heat up the machine and dry and energy recovery of the packaging.
the incoming waste)
4 Environmental Product Declaration - PROMAT - Monalite® M1AT and Monalite® M1T
5. LCA: Results
Note that module A5 only waste treatment of the packaging of the final product includes. Installation itself has not been included, as a
wide variety exists depending on the application.
Note that both 100 % recycling (scenario 1) and 100 % landfill (scenario 2) scenarios have been calculated.
DESCRIPTION OF THE SYSTEM BOUNDARY (X = INCLUDED IN LCA; ND = MODULE OR INDICATOR NOT DECLARED; MNR =
MODULE NOT RELEVANT)
Benefits and
Construction loads beyond
Product stage Use stage End of life stage
process stage the system
boundaries
la ire ta m w a Ry lp p u s tro p s n a rT g n iru tc a fu n a M e h t m o rf tro p s n a rTe tis e h t o t e ta g y lb m e s s A e s U e c n a n e tn ia M ria p e R tn e m e c a lp e R tn e m h s ib ru fe R y g re n e la n o ita re p Oe s u re ta w la n o ita re p Oe s u n o itc u rts n o c -e Dn o itilo m e d tro p s n a rT g n is s e c o rp e ts a W la s o p s iD -e s u e R-y re v o c e R-g n ilc y c e Rla itn e to p
A1 A2 A3 A4 A5 B1 B2 B3 B4 B5 B6 B7 C1 C2 C3 C4 D
X X X MND X MND MND MNR MNR MNR MND MND MND X X X X
RESULTS OF THE LCA - ENVIRONMENTAL IMPACT according to EN 15804+A2: 1 m^2 Monalite® M1AT/Monalite® M1T
Parameter Unit A1-A3 A5 C2/1 C2/2 C3/1 C3/2 C4/1 C4/2 D/1 D/2
GWP-total kg CO 2 eq 4.51E+01 6.26E-01 3.57E-01 3.19E-01 2.98E+00 0 0 2.74E+00 -9.02E-01 -2.72E-01
GWP-fossil kg CO 2 eq 4.92E+01 1.63E-02 3.56E-01 3.19E-01 4.64E-01 0 0 2.32E-01 -6.91E-01 -6.22E-02
GWP-
biogenic kg CO 2 eq -4.15E+00 6.09E-01 1.28E-04 1.14E-04 2.51E+00 0 0 2.51E+00 -2.11E-01 -2.09E-01
GWP-luluc kg CO 2 eq 1.32E-02 5.39E-06 1.43E-04 1.27E-04 1.01E-03 0 0 1.71E-04 -8.74E-04 -2.68E-04
ODP kg CFC11 eq 5.76E-06 2.73E-09 8.26E-08 7.38E-08 3.42E-08 0 0 8.58E-08 -8E-08 -7.33E-09
AP mol H+ eq 1.9E-01 8.06E-05 1.01E-03 9.05E-04 3.04E-03 0 0 2.04E-03 -3.82E-03 -2.72E-04
EP-
kg P eq 3.52E-04 1.51E-07 2.54E-06 2.27E-06 4.55E-05 0 0 7.11E-06 -3.1E-05 -4.26E-06
freshwater
EP-marine kg N eq 5.21E-02 3.3E-05 2.01E-04 1.8E-04 6.33E-04 0 0 6.98E-04 -9.87E-04 -6.79E-05
EP-terrestrial mol N eq 5.67E-01 3.29E-04 2.24E-03 2E-03 7.16E-03 0 0 7.7E-03 -1.31E-02 -7.46E-04
kg NMVOC
POCP 1.58E-01 9.72E-05 8.62E-04 7.7E-04 1.91E-03 0 0 2.19E-03 -3.08E-03 -2.54E-04
eq
ADPE kg Sb eq 4.51E-05 3.24E-08 9.65E-07 8.63E-07 1.01E-06 0 0 5.49E-07 -1.71E-06 -1.7E-07
ADPF MJ 6.02E+02 1.92E-01 5.4E+00 4.83E+00 9.41E+00 0 0 6.62E+00 -1.25E+01 -1.14E+00
m3 world eq
WDP 2.21E+00 1.08E-03 1.65E-02 1.47E-02 1.19E-01 0 0 3.1E-02 -1.03E-01 -3.38E-02
deprived
GWP = Global warming potential; ODP = Depletion potential of the stratospheric ozone layer; AP = Acidification potential of land and water; EP =
Eutrophication potential; POCP = Formation potential of tropospheric ozone photochemical oxidants; ADPE = Abiotic depletion potential for non-fossil
resources; ADPF = Abiotic depletion potential for fossil resources; WDP = Water (user) deprivation potential)
RESULTS OF THE LCA - INDICATORS TO DESCRIBE RESOURCE USE according to EN 15804+A2: 1 m^2 Monalite®
M1AT/Monalite® M1T
Parameter Unit A1-A3 A5 C2/1 C2/2 C3/1 C3/2 C4/1 C4/2 D/1 D/2
PERE MJ 1.95E+02 1.65E+00 7.6E-02 6.79E-02 1.38E+00 0 0 3.42E-01 0 0
PERM MJ 3.7E+01 -3.64E+00 0 0 -2.19E+01 0 0 0 2.39E+01 1.99E+00
PERT MJ 2.32E+02 -1.99E+00 7.6E-02 6.79E-02 -2.03E+01 0 0 3.42E-01 2.39E+01 1.99E+00
PENRE MJ 6.67E+02 2.36E-01 5.43E+00 4.86E+00 9.56E+00 0 0 6.79E+00 0 0
PENRM MJ 9.82E-02 -6E-02 0 0 0 0 0 0 2.83E-02 2.83E-02
PENRT MJ 6.68E+02 1.68E-01 5.43E+00 4.86E+00 1.12E+01 0 0 6.79E+00 2.83E-02 2.83E-02
SM kg 6E-03 0 0 0 0 0 0 0 0 0
RSF MJ 0 0 0 0 0 0 0 0 0 0
NRSF MJ 0 0 0 0 0 0 0 0 0 0
FW m3 1.26E+00 1.12E-04 3.97E-04 3.55E-04 7.78E-03 0 0 7.11E-03 -5.83E-03 -9.95E-04
PERE = Use of renewable primary energy excluding renewable primary energy resources used as raw materials; PERM = Use of renewable primary
energy resources used as raw materials; PERT = Total use of renewable primary energy resources; PENRE = Use of non-renewable primary energy
excluding non-renewable primary energy resources used as raw materials; PENRM = Use of non-renewable primary energy resources used as raw
materials; PENRT = Total use of non-renewable primary energy resources; SM = Use of secondary material; RSF = Use of renewable secondary fuels;
NRSF = Use of non-renewable secondary fuels; FW = Use of net fresh water
RESULTS OF THE LCA – WASTE CATEGORIES AND OUTPUT FLOWS according to EN 15804+A2:
1 m^2 Monalite® M1AT/Monalite® M1T
Parameter Unit A1-A3 A5 C2/1 C2/2 C3/1 C3/2 C4/1 C4/2 D/1 D/2
HWD kg 9.07E-04 4.43E-07 1.41E-05 1.26E-05 5.03E-06 0 0 7.25E-06 -1.5E-05 -1.53E-06
NHWD kg 1.29E+01 1.51E-01 2.83E-01 2.53E-01 6.02E-02 0 0 3.82E+01 -3.24E-02 -8.41E-03
RWD kg 1.12E-03 1.24E-06 3.65E-05 3.26E-05 6.77E-05 0 0 4.52E-05 -5.16E-05 -4.82E-06
5 Environmental Product Declaration - PROMAT - Monalite® M1AT and Monalite® M1T
CRU kg 0 0 0 0 0 0 0 0 0 0
MFR kg 0 1.39E-01 0 0 3.82E+01 0 0 0 0 0
MER kg 0 0 0 0 0 0 0 0 0 0
EEE MJ 0 1.68E-01 0 0 0 0 0 0 0 0
EET MJ 0 3.35E-01 0 0 0 0 0 0 0 0
HWD = Hazardous waste disposed; NHWD = Non-hazardous waste disposed; RWD = Radioactive waste disposed; CRU = Components for re-use;
MFR = Materials for recycling; MER = Materials for energy recovery; EEE = Exported electrical energy; EET = Exported thermal energy
RESULTS OF THE LCA – additional impact categories according to EN 15804+A2-optional:
1 m^2 Monalite® M1AT/Monalite® M1T
Parameter Unit A1-A3 A5 C2/1 C2/2 C3/1 C3/2 C4/1 C4/2 D/1 D/2
Disease
PM 7.17E-07 1.39E-09 2.86E-08 2.56E-08 1.42E-08 0 0 3.96E-08 -3.92E-08 -5.89E-09
incidence
IR kBq U235 eq 8.29E-01 8.6E-04 2.35E-02 2.1E-02 8.16E-02 0 0 3.38E-02 -5.65E-02 -5.16E-03
ETP-fw CTUe 3.08E+02 1.76E-01 4.24E+00 3.79E+00 8.73E+00 0 0 3.8E+00 -8.56E+01 -7.48E-01
HTP-c CTUh 8.45E-09 4.02E-11 1.36E-10 1.22E-10 6.88E-10 0 0 1.1E-10 -1.89E-10 -3.03E-11
HTP-nc CTUh 2.11E-07 2.54E-10 4.29E-09 3.83E-09 7.8E-09 0 0 2.23E-09 -5E-09 -7.05E-10
SQP SQP 4.46E+02 1.87E-01 3.77E+00 3.37E+00 2.04E+00 0 0 1.25E+01 -2.49E+01 -2.33E+01
PM = Potential incidence of disease due to PM emissions; IR = Potential Human exposure efficiency relative to U235; ETP-fw = Potential comparative
Toxic Unit for ecosystems; HTP-c = Potential comparative Toxic Unit for humans (cancerogenic); HTP-nc = Potential comparative Toxic Unit for humans
(not cancerogenic); SQP = Potential soil quality index
Disclaimer 1 – for the indicator “Potential Human exposure efficiency relative to U235”. This impact category deals mainly with the
eventual impact of low-dose ionizing radiation on human health of the nuclear fuel cycle. It does not consider effects due to possible
nuclear accidents, occupational exposure or radioactive waste disposal in underground facilities. Potential ionizing radiation from the
soil, radon and from some construction materials is also not measured by this indicator.
Disclaimer 2 – for the indicators “abiotic depletion potential for non-fossil resources”, “abiotic depletion potential for fossil resources”,
“water (user) deprivation potential, deprivation-weighted water consumption”, “potential comparative toxic unit for ecosystems”,
“potential comparative toxic unit for humans – cancerogenic”, “Potential comparative toxic unit for humans - not cancerogenic”,
“potential soil quality index”. The results of this environmental impact indicator shall be used with care as the uncertainties on these
results are high as there is limited experience with the indicator.
6. LCA: Interpretation
The environmental profile shows the contribution of the various highest contribution on all impact categories. Also, the transport
steps in the life cycle, per environmental impact category. For of the raw materials to the factory is significant for several
the declared products produced in Belgium, the manufacturing impact indicators.
stage and raw materials used in the formulation mix have the
7. Requisite evidence
8. References
Standards
EN 16757:2017, Sustainability of construction works–
EN 12467 Environmental product declarations – Product Category
Rulesfor concrete and concrete elements
EN 12467:2012+A2:2018, Fibre-cement flat sheets. Product
specification and test methods ISO 9001
EN 13501-1 ISO 9001:2015: Quality management systems — Requirements
DIN EN 13501-1:2019-05: Fire classification of ISO 14001
constructionproducts and building elements - Part 1:
classification usingdata from reaction to fire tests ISO 14001:2015: Environmental management systems —
Requirements with guidance for use
EN 14306
ISO 14025
EN 14306:2009+A1:2013, Thermal insulation products
forbuilding equipment and industrial installations. Factory EN ISO 14025:2011, Environmental labels and declarations —
madecalcium silicate (CS) products. Specification Type III environmental declarations — Principles
andprocedures.
EN 15804
ISO 14040
EN 15804:2012+A2:2019+AC:2021, Sustainability of
construction works — Environmental Product Declarations — ISO 14040:2006: Environmental management – Life
Core rules for the product category of construction products. cycleassessment –Principles and framework.
EN 16757 ISO 14044
6 Environmental Product Declaration - PROMAT - Monalite® M1AT and Monalite® M1T
ISO 14044:2006: Environmental management – Life cycle Ordinance on Biocide Products No. 528/2012
assessment – Requirements and guidelines.
Biocidal Products Regulation (BPR, Regulation (EU) 528/2012)
ISO 45001
PEFCR
ISO 45001:2018:Occupational health and safety management
systems Requirements with guidance for use European commission (2018). Product Environmental Footprint
Category Rules PEFCR Guidance, version 6.3.
Further references
PCR Part A
CPR
Calculation rules for the Life Cycle Assessment and
European Regulation N° 305/2011 (CPR) Requirements on the Background Report, Institut Bauen und
Umwelt e.V., www.bauumwelt.com.
ECHA candidate list
PCR Part B
Candidate List of substances of very high concern (SVHCs) for
authorisation, last update 26.07.2022, European Chemicals Institut Bauen und Umwelt e.V, Berlin (pub.): PCR Guidance
Agency (ECHA), Helsinki, Finland Texts for Building-Related Products and Services From the
range of Environmental Product Declarations of Institute
Ecoinvent Construction and Environment e.V. (IBU) : Requirements on the
EPD for Calcium silicate insulating materials
Wernet, G., Bauer, C., Steubing, B., Reinhard, J., Moreno-
Ruiz,E., and Weidema, B., 2016. The ecoinvent database Pré Consultants (2021)
version 3 (part I): overview and methodology. The International
Journal of Life Cycle Assessment, [online] 21(9), pp.1218– SimaPro 9.2.0.1 [Computer Software]. Amersfoort, The
1230. Availableat:http://link.springer.com/10.1007/s11367-016- Netherlands.
1087-8.
REACH
Enperas
Regulation (EC) No 1907/2006 of the European Parliament and
Quadrant tool. 2023. Genk, Belgium of the Council of 18 December 2006 concerning the
Registration, Evaluation, Authorisation and Restriction of
European Waste Code Chemicals (REACH), June 2017
Commission of the European Communities, 2010, Guidance
onclassification of waste according to EWC-Stat categories
IBU
IBU 2021. Institut Bauen und Umwelt e.V.: General Instructions
for the EPD programme of Institut Bauen und Umwelt e.V.,
Version 2.0, Berlin: Institut Bauen und Umwelt e.V., 2021
www.ibu-epd.com The literature referred to in the Environmental Product
Declaration must be listed in full.Standards already fully quoted
Industry 2.0 in the EPD do not need to be listed here again.
The current version of PCR Part A and PCR Part B of the PCR
Industry 2.0 (from PlasticsEurope, worldsteel and ERASM). document on which they are based must be referenced.
LCA database as integrated in SimaPro 9.3.0.3.
7 Environmental Product Declaration - PROMAT - Monalite® M1AT and Monalite® M1T
Publisher
Institut Bauen und Umwelt e.V. +49 (0)30 3087748- 0
Hegelplatz 1 info@ibu-epd.com
10117 Berlin www.ibu-epd.com
Germany
Programme holder
Institut Bauen und Umwelt e.V. +49 (0)30 3087748- 0
Hegelplatz 1 info@ibu-epd.com
10117 Berlin www.ibu-epd.com
Germany
Author of the Life Cycle Assessment
Enperas +32 3 376 00 19
Thorpark 8300 info@enperas.com
3600 Genk https://www.enperas.com/en/
Belgium
Owner of the Declaration
Etex Building Performance International +32 2 778 12 11
Rue Marcel Demonque 500 info@etexgroup.com
84915 Avignon Cedex 9 www.etexgroup.com
France
8 Environmental Product Declaration - PROMAT - Monalite® M1AT and Monalite® M1T
