ENVIRONMENTAL PRODUCT DECLARATION
as per ISO 14025 and EN 15804+A2
Owner of the Declaration Etex Building Performance International
Publisher Institut Bauen und Umwelt e.V. (IBU)
Programme holder Institut Bauen und Umwelt e.V. (IBU)
Declaration number EPD-ETE-20230252-IBA1-EN
Issue date 25/09/2023
Valid to 24/09/2028
Monolux®
PROMAT
www.ibu-epd.com | https://epd-online.com
1. General Information
PROMAT Monolux®
Programme holder Owner of the declaration
IBU – Institut Bauen und Umwelt e.V. Etex Building Performance International
Hegelplatz 1 Rue Marcel Demonque 500
10117 Berlin 84915 Avignon Cedex 9
Germany France
Declaration number Declared product / declared unit
EPD-ETE-20230252-IBA1-EN 1 m2 of Monolux® with a thickness of 38.5 mm
This declaration is based on the product category rules: Scope:
Calcium silicate insulating materials, 01/08/2021 This EPD is representative and relevant for Monolux® boards produced by
(PCR checked and approved by the SVR) ETEX in Tisselt (Belgium) and installed in Europe. The data describing the
direct inputs and outputs of the foreground processes are representative
for ETEX production in Tisselt, Belgium, and taken from the period of one
Issue date year between October 2020 and September 2021.
25/09/2023
The owner of the declaration shall be liable for the underlying information
and evidence; the IBU shall not be liable with respect to manufacturer
information, life cycle assessment data and evidences.
Valid to
24/09/2028 The EPD was created according to the specifications of EN 15804+A2. In
the following, the standard will be simplified as EN 15804.
Verification
The standard EN 15804 serves as the core PCR
Independent verification of the declaration and data according to ISO
14025:2011
internally X externally
Dipl.-Ing. Hans Peters
(Chairman of Institut Bauen und Umwelt e.V.)
Florian Pronold Vito D'Incognito,
(Managing Director Institut Bauen und Umwelt e.V.) (Independent verifier)
1 Environmental Product Declaration - PROMAT - Monolux®
2. Product
The main constituents of the product are silica (10-25 %),
2.1 Product description/Product definition wollastonite (20-35 %), cement (1-10 %), lime (10-30 %) and
This EPD describes the life cycle analysis of MONOLUX® for cellulose fibres (1-10 %).
fire protection in heavy industries. It is the cement-bounded
calcium silicate board with increased density. MONOLUX® This product/article/at least one partial article contains
materials are rigid insulation boards with a low thermal substances listed in the candidate list (date: accesses
conductivity. They are specifically formulated without asbestos 31/07/2023) exceeding 0.1 percentage by mass: no
and mineral fibres. MONOLUX® products have low shrinkage
and high strength and therefore provide effective and stable This product/article/at least one partial article contains other
insulation solutions for industrial applications. MONOLUX® carcinogenic, mutagenic, reprotoxic (CMR) substances in
boards combine high mechanical strength, good thermal and categories 1A or 1B which are not on the candidate list,
electric insulation at high temperatures. exceeding 0.1 percentage by mass: no
Product according to the CPR based on a hEN: Biocide products were added to this construction product or it
For the placing on the market of the product in the European has been treated with biocide products (this then concerns a
Union/European Free Trade Association (EU/EFTA) (with the treated product as defined by the (EU) Ordinance on Biocide
exception of Switzerland) Regulation (EU) No. 305/2011 (CPR) Products No. 528/2012): no
applies. The product needs a declaration of performance taking
into consideration EN 14306:2009+A1:2013 and No. 0432- 2.6 Manufacture
CPR-00541-01 - 2020/5, MONOLUX® and the CE-marking. For There is only one manufacturing plant of the declared products,
the application and use the respective national provisions apply. being the manufacturing plant in Tisselt (Belgium). The
products are all produced on the same type of production line.
2.2 Application All raw materials, including previously made xonotlite slurries,
Monolux® boards are versatile multi-purpose fire protection together with a balanced amount of water are mixed to form a
boards, for multiple applications: slurry, and shaped by a filter press to produce a wet board. It is
steam cured in an autoclave to form required calcium silicate
OIL AND GAS minerals suitable for the end application. The final steps are
• Load bearing pipe supports drying, cutting and sanding/finishing. During the cutting and
• Heat shields finishing, scrap is produced which is partly recycled, both
HEAVY INDUSTRY internally and externally, and partly landfilled.
• Structural thermal separations 2.7 Environment and health during manufacturing
• Furnace bottom boards Environmental, occupational health, safety and quality
• Dryer walls management at the Guangzhou plant are in accordance with
the following standards:
2.3 Technical Data
· ISO 14001;2015
Constructional data · ISO 9001;2015
Name Value Unit · ISO 45001:2018
Gross density EN12467 950 kg/m3 2.8 Product processing/Installation
Compressive strength EN 993-5 2000 (cold) >27 N/mm2 Not considered in the EPDs. Various installation scenarios exist
Flexural strength EN 993-6 1995 >7.0 N/mm2 depending on the application.
Thermal conductivity at 200°C 0.20 W/(mK)
2.9 Packaging
Thermal conductivity at 400°C 0.21 W/(mK) The products are transported and delivered on a wooden pallet
Thermal conductivity at 600°C 0.22 W/(mK) and packed with cartons and PET straps.
Thermal conductivity at 800°C 0.23 W/(mK)
2.10 Condition of use
B modules are not included. These products are designed for
Product according to the CPR based on a hEN:
life and depending on the application in which the products are
For the placing on the market of the product in the European
used there might be a need for
Union/European Free Trade Association (EU/EFTA) (with the
maintenance/repair/replacement of the application.
exception of Switzerland) Regulation (EU) No. 305/2011 (CPR)
applies. The product needs a declaration of performance taking 2.11 Environment and health during use
into consideration EN 14306:2009+A1:2013 and No. 0432- Under normal conditions of use, the products do not cause any
CPR-00541-01 - 2020/5, MONOLUX® and the CE-marking. For adverse health effects or release of volatile organic compounds
the application and use the respective national provisions apply. (VOCs) into indoor air. No environmental impact on water, air or
soil is expected due to the extremely low metal release from the
2.4 Delivery status
low maintenance requirements.
The products have a thickness of 12.7, 20, 25, 30, 40, 50 or 60
mm. 2.12 Reference service life
The length is 2500 mm. The RSL depends on the application. Under normal conditions
The width is 1200 mm. of use, the product is supposed to remain its characteristics as
long as the application lasts. For application in building a
The products are transported and delivered on a wooden pallet reference service life of 60 years (i.e life time of the building)
and packed with cartons and PET straps. could be declared.
2.5 Base materials/Ancillary materials 2.13 Extraordinary effects
2 Environmental Product Declaration - PROMAT - Monolux®
Fire In case of mechanical destruction, no risks are expected to
Information on the fire performance according to EN 13501:1. occur in terms of environment and human health.
Fire protection
2.14 Re-use phase
Name Value Currently, the boards can be recycled as a replacement of filler
Building material class A1 (e.g. secondary limestone fillers). In the EPD, both the 100 %
Burning droplets / recycling and 100 % landfill scenario have been calculated.
Smoke gas development /
2.15 Disposal
The waste number according to the European list 'Decision N°
Water 2000/532/CE' is '17 09 00: other construction and demolition
Tests on the product performance including possible impacts on wastes'.
the environment following the unforeseeable influence of water,
e.g. flooding showed that no risks are expected to occur in 2.16 Further information
terms of environment and human health. https://www.promat.com/en/industry/products-solutions/high-
temperature-insulation/boards-hti/monolux/
Mechanical destruction
3. LCA: Calculation rules
3.1 Declared Unit 3.5 Background data
1 m2 of Monolux® with a thickness of 38.5 mm. Ecoinvent 3.8 and Industry 2.0
Declared unit 3.6 Data quality
Name Value Unit Company-specific data concern the data about the production
Declared unit 1 m² of Monolux®. All required data about the production process
Gross density 950 kg/m3 have been delivered to Enperas by ETEX.
Grammage 36.58 kg/m2
The composed datasets for this project are representative and
Conversion factor to 1 kg 0.027 relevant for Monolux® produced by ETEX in Tisselt, Belgium.
Layer thickness 0.0385 m
3.7 Period under review
Assuming a linear relationship between the thickness and the
The data collected by ETEX are based on data from the period
mass/environmental impact of the board, the environmental
of one year between October 2020 and September 2021.
impact of a product can be considered to be proportional to the
thickness of the product, so products with another thickness 3.8 Geographic Representativeness
can be calculated by the below formula: Land or region, in which the declared product system is
manufactured, used or handled at the end of the product´s
E=W*Eref/Wref lifespan: Europe
E=environmental impact of a product with density d and
thickness t 3.9 Allocation
W=d*t=weight of 1 m2 product with density d and thickness t No co-products are produced.
Eref=environmental impact of the reference product No secondary raw materials are used.
Wref=weight of 1 m2 reference product At ETEX's plant in Tisselt, different types of calcium silicate
boards are produced. For most of the production data, product
specific data is available, as the data per production step or
product line could be extracted. In this case, the data have
3.2 System boundary been allocated to the declared unit using the annual production
Cradle-to-gate with options, including modules C2-C4 and D volume of that product in m2.5 (i.e. 1 m2 with a thickness of 5
mm is the reference unit in ETEX's factory). The last step was
3.3 Estimates and assumptions
to recalculate the amount to the declared unit by multiplying
Nothing to declare. with the mass ratio between 1 m2.5 and 1 m2 with the thickness
declared in the EPD. This approach has been used for all
3.4 Cut-off criteria
inputs and outputs, except for water use/discharge and
The following processes are considered below cut-off according
production waste-externally recycled. For the water
to the rules as per the PCR, Part A:
use/discharge, only facility-level data were available. These
• Packaging of raw materials, as the main raw materials have been allocated to the individual product using the annual
(i.e. largest amounts) come in bulk. production volume in kg. For the production waste-externally
• Ancillary materials for production recycled, facility-level data were available for all the declared
• Infrastructure and land use of the factory products together with two other Promat products of the Tisselt
• Environmental impacts caused by the personnel of the plant. These have been allocated to the individual product using
production plants are not included in the LCA, e.g. the annual production volume in kg.
waste from the cafeteria and sanitary installations,
accidental pollution caused by human mistakes, or 3.10 Comparability
environmental effects caused by commuter traffic.
Basically, a comparison or an evaluation of EPD data is only
Heating or cooling of the plants in order to ensure a
possible if all the data sets to be compared were created
comfortable indoor climate for the personnel for
according to EN 15804 and the building context, respectively
example is also neglected.
the product-specific characteristics of performance, are taken
3 Environmental Product Declaration - PROMAT - Monolux®
into account. Ecoinvent 3.8 and Industry 2.0
4. LCA: Scenarios and additional technical information
the incoming waste).
Characteristic product properties of biogenic carbon 3. the remaining powder (<100µm) will be used as a filler
The Promat boards contain biogenic carbon in the form of replacing limestone in cement applications
cellulose (assumed 0,44 kg C/kg cellulose). Also, its packaging Name ValueUnit
contains biogenic carbon in the form of cartons (assumed 0,44
Collected as mixed construction waste 36.58 kg
kg C/kg carton) and wooden pallets (assumed 0,45 kg C/kg
Recycling Scenario 1 (cellulose content is
wood). 36.58 kg
incinerated)
Information on describing the biogenic carbon content at
Landfilling Scenario 2 36.58 kg
factory gate
Reuse, recovery and/or recycling potentials (D), relevant
Name ValueUnit
scenario information
kg
Biogenic carbon content in product 1.14
C
In module D, the benefits and loads beyond the system
Biogenic carbon content in accompanying 0.788 kg boundaries are quantified. For recycling, it concerns both the
packaging C loads of the recycling processes after the end-of-waste and the
benefits of the avoided virgin materials, when the recycled
components are used for other purposes. In case of
incineration, it concerns the benefits from the avoided
End of life (C1-C4)
production of energy grace to energy recovery.
In the EPD both 100 % recycling and 100 % landfill scenarios
have been calculated. Recycling consists in
Benefits of recycling the product in limestone production have
been included in module D (avoided impact of limestone
1. milling/crushing the boards production and energy recovery from incineration of cellulose),
2. sieving out the fibres which will be incinerated and used together with some minor benefits and loads due to recycling
as an energy source (to heat up the machine and dry and energy recovery of the packaging.
4 Environmental Product Declaration - PROMAT - Monolux®
5. LCA: Results
Note that module A5 only waste treatment of the packaging of the final product includes. Installation itself has not been included, as a
wide variety exists depending on the application.
Note that both 100 % recycling (scenario 1) and 100 % landfill (scenario 2) scenarios have been calculated.
DESCRIPTION OF THE SYSTEM BOUNDARY (X = INCLUDED IN LCA; ND = MODULE OR INDICATOR NOT DECLARED; MNR =
MODULE NOT RELEVANT)
Benefits and
Construction loads beyond
Product stage Use stage End of life stage
process stage the system
boundaries
la ire ta m w a Ry lp p u s tro p s n a rT g n iru tc a fu n a M e h t m o rf tro p s n a rTe tis e h t o t e ta g y lb m e s s A e s U e c n a n e tn ia M ria p e R tn e m e c a lp e R tn e m h s ib ru fe R y g re n e la n o ita re p Oe s u re ta w la n o ita re p Oe s u n o itc u rts n o c -e Dn o itilo m e d tro p s n a rT g n is s e c o rp e ts a W la s o p s iD -e s u e R-y re v o c e R-g n ilc y c e Rla itn e to p
A1 A2 A3 A4 A5 B1 B2 B3 B4 B5 B6 B7 C1 C2 C3 C4 D
X X X MND X MND MND MNR MNR MNR MND MND MND X X X X
RESULTS OF THE LCA - ENVIRONMENTAL IMPACT according to EN 15804+A2: 1 m^2 Monolux®
Parameter Unit A1-A3 A5 C2/1 C2/2 C3/1 C3/2 C4/1 C4/2 D/1 D/2
GWP-total kg CO 2 eq 2.52E+01 1.14E+00 3.78E-01 3.11E-01 4.87E+00 0 0 4.62E+00 -1.54E+00 -4.98E-01
GWP-fossil kg CO 2 eq 3.22E+01 3.03E-02 3.78E-01 3.11E-01 4.61E-01 0 0 2.22E-01 -1.15E+00 -1.13E-01
GWP-
biogenic kg CO 2 eq -7.08E+00 1.1E+00 1.35E-04 1.11E-04 4.4E+00 0 0 4.4E+00 -3.87E-01 -3.84E-01
GWP-luluc kg CO 2 eq 1.09E-02 9.81E-06 1.51E-04 1.24E-04 9.66E-04 0 0 1.64E-04 -1.53E-03 -4.86E-04
ODP kg CFC11 eq 3.67E-06 4.97E-09 8.75E-08 7.21E-08 4.07E-08 0 0 8.21E-08 -1.29E-07 -1.34E-08
AP mol H+ eq 1.19E-01 1.46E-04 1.07E-03 8.83E-04 3.36E-03 0 0 1.96E-03 -5.14E-03 -5E-04
EP-
kg P eq 2.88E-04 2.74E-07 2.69E-06 2.22E-06 4.31E-05 0 0 6.8E-06 -5.42E-05 -7.75E-06
freshwater
EP-marine kg N eq 3.15E-02 5.95E-05 2.13E-04 1.76E-04 8.21E-04 0 0 6.68E-04 -1.18E-03 -1.26E-04
EP-terrestrial mol N eq 3.39E-01 5.93E-04 2.38E-03 1.96E-03 9.25E-03 0 0 7.37E-03 -1.51E-02 -1.38E-03
kg NMVOC
POCP 9.51E-02 1.75E-04 9.13E-04 7.52E-04 2.44E-03 0 0 2.1E-03 -3.77E-03 -4.67E-04
eq
ADPE kg Sb eq 2.37E-05 5.89E-08 1.02E-06 8.42E-07 1.09E-06 0 0 5.26E-07 -2.84E-06 -3.13E-07
ADPF MJ 3.58E+02 3.48E-01 5.73E+00 4.72E+00 9.03E+00 0 0 6.34E+00 -2.13E+01 -2.08E+00
m3 world eq
WDP 2.27E+00 1.95E-03 1.74E-02 1.44E-02 1.27E-01 0 0 2.97E-02 -1.81E-01 -6.6E-02
deprived
GWP = Global warming potential; ODP = Depletion potential of the stratospheric ozone layer; AP = Acidification potential of land and water; EP =
Eutrophication potential; POCP = Formation potential of tropospheric ozone photochemical oxidants; ADPE = Abiotic depletion potential for non-fossil
resources; ADPF = Abiotic depletion potential for fossil resources; WDP = Water (user) deprivation potential)
RESULTS OF THE LCA - INDICATORS TO DESCRIBE RESOURCE USE according to EN 15804+A2: 1 m^2 Monolux®
Parameter Unit A1-A3 A5 C2/1 C2/2 C3/1 C3/2 C4/1 C4/2 D/1 D/2
PERE MJ 7.25E+01 2.97E+00 8.05E-02 6.63E-02 1.3E+00 0 0 3.27E-01 0 0
PERM MJ 6.27E+01 -6.62E+00 0 0 -3.84E+01 0 0 0 4.21E+01 3.67E+00
PERT MJ 1.35E+02 -3.66E+00 8.05E-02 6.63E-02 -3.69E+01 0 0 3.27E-01 4.21E+01 3.67E+00
PENRE MJ 3.95E+02 4.32E-01 5.76E+00 4.74E+00 9.19E+00 0 0 6.5E+00 0 0
PENRM MJ 1.93E-01 -1.18E-01 0 0 0 0 0 0 5.57E-02 5.57E-02
PENRT MJ 3.95E+02 3.01E-01 5.76E+00 4.74E+00 1.07E+01 0 0 6.5E+00 5.57E-02 5.57E-02
SM kg 2.7E-02 0 0 0 0 0 0 0 0 0
RSF MJ 0 0 0 0 0 0 0 0 0 0
NRSF MJ 0 0 0 0 0 0 0 0 0 0
FW m3 2.88E-01 2.02E-04 4.21E-04 3.47E-04 8.12E-03 0 0 6.81E-03 -9.64E-03 -1.91E-03
PERE = Use of renewable primary energy excluding renewable primary energy resources used as raw materials; PERM = Use of renewable primary
energy resources used as raw materials; PERT = Total use of renewable primary energy resources; PENRE = Use of non-renewable primary energy
excluding non-renewable primary energy resources used as raw materials; PENRM = Use of non-renewable primary energy resources used as raw
materials; PENRT = Total use of non-renewable primary energy resources; SM = Use of secondary material; RSF = Use of renewable secondary fuels;
NRSF = Use of non-renewable secondary fuels; FW = Use of net fresh water
RESULTS OF THE LCA – WASTE CATEGORIES AND OUTPUT FLOWS according to EN 15804+A2:
1 m^2 Monolux®
Parameter Unit A1-A3 A5 C2/1 C2/2 C3/1 C3/2 C4/1 C4/2 D/1 D/2
HWD kg 4.64E-04 8.04E-07 1.49E-05 1.23E-05 5.38E-06 0 0 6.94E-06 -2.41E-05 -2.79E-06
NHWD kg 6.58E+00 2.73E-01 3E-01 2.47E-01 7.97E-02 0 0 3.66E+01 -5.5E-02 -1.56E-02
RWD kg 8.47E-04 2.25E-06 3.87E-05 3.19E-05 6.38E-05 0 0 4.33E-05 -8.57E-05 -8.76E-06
CRU kg 0 0 0 0 0 0 0 0 0 0
5 Environmental Product Declaration - PROMAT - Monolux®
MFR kg 0 2.56E-01 0 0 3.66E+01 0 0 0 0 0
MER kg 0 0 0 0 0 0 0 0 0 0
EEE MJ 0 3.02E-01 0 0 0 0 0 0 0 0
EET MJ 0 6.04E-01 0 0 0 0 0 0 0 0
HWD = Hazardous waste disposed; NHWD = Non-hazardous waste disposed; RWD = Radioactive waste disposed; CRU = Components for re-use;
MFR = Materials for recycling; MER = Materials for energy recovery; EEE = Exported electrical energy; EET = Exported thermal energy
RESULTS OF THE LCA – additional impact categories according to EN 15804+A2-optional:
1 m^2 Monolux®
Parameter Unit A1-A3 A5 C2/1 C2/2 C3/1 C3/2 C4/1 C4/2 D/1 D/2
Disease
PM 5.84E-07 2.51E-09 3.03E-08 2.5E-08 1.73E-08 0 0 3.79E-08 -4.56E-08 -1.09E-08
incidence
IR kBq U235 eq 6.38E-01 1.56E-03 2.49E-02 2.05E-02 7.67E-02 0 0 3.24E-02 -9.63E-02 -9.35E-03
ETP-fw CTUe 2.74E+02 3.22E-01 4.49E+00 3.7E+00 1.13E+01 0 0 3.64E+00 -8.27E+01 -1.38E+00
HTP-c CTUh 6.29E-09 7.25E-11 1.45E-10 1.19E-10 1.08E-09 0 0 1.06E-10 -3.08E-10 -5.54E-11
HTP-nc CTUh 1.52E-07 4.61E-10 4.54E-09 3.74E-09 1.02E-08 0 0 2.14E-09 -8.08E-09 -1.29E-09
SQP SQP 6.99E+02 3.37E-01 3.99E+00 3.29E+00 2E+00 0 0 1.2E+01 -4.5E+01 -4.28E+01
PM = Potential incidence of disease due to PM emissions; IR = Potential Human exposure efficiency relative to U235; ETP-fw = Potential comparative
Toxic Unit for ecosystems; HTP-c = Potential comparative Toxic Unit for humans (cancerogenic); HTP-nc = Potential comparative Toxic Unit for humans
(not cancerogenic); SQP = Potential soil quality index
Disclaimer 1 – for the indicator “Potential Human exposure efficiency relative to U235”. This impact category deals mainly with the
eventual impact of low-dose ionizing radiation on human health of the nuclear fuel cycle. It does not consider effects due to possible
nuclear accidents, occupational exposure or radioactive waste disposal in underground facilities. Potential ionizing radiation from the
soil, radon and from some construction materials is also not measured by this indicator.
Disclaimer 2 – for the indicators “abiotic depletion potential for non-fossil resources”, “abiotic depletion potential for fossil resources”,
“water (user) deprivation potential, deprivation-weighted water consumption”, “potential comparative toxic unit for ecosystems”,
“potential comparative toxic unit for humans – cancerogenic”, “Potential comparative toxic unit for humans - not cancerogenic”,
“potential soil quality index”. The results of this environmental impact indicator shall be used with care as the uncertainties on these
results are high as there is limited experience with the indicator.
6. LCA: Interpretation
The environmental profile shows the contribution of the various highest contribution on all impact categories. Also, the transport
steps in the life cycle, per environmental impact category. For of the raw materials to the factory is significant for several
the declared products produced in Belgium, the manufacturing impact indicators.
stage and raw materials used in the formulation mix have the
7. Requisite evidence
8. References
Standards EN 16757:2017, Sustainability of construction works–
Environmental product declarations – Product Category Rules
EN 12467 for concrete and concrete elements
EN 12467:2012+A2:2018, Fibre-cement flat sheets. Product ISO 9001
specification and test methods
ISO 9001:2015: Quality management systems — Requirements
EN 13501-1
ISO 14001
DIN EN 13501-1:2019-05: Fire classification of construction
products and building elements - Part 1: classification using ISO 14001:2015: Environmental management systems —
data from reaction to fire tests Requirements with guidance for use
EN 14306 ISO 14025
EN 14306:2009+A1:2013, Thermal insulation products for EN ISO 14025:2011, Environmental labels and declarations —
building equipment and industrial installations. Factory made Type III environmental declarations — Principles and
calcium silicate (CS) products. Specification procedures.
EN 15804 ISO 14040
EN 15804:2012+A2:2019+AC:2021, Sustainability of ISO 14040:2006: Environmental management – Life cycle
construction works — Environmental Product Declarations — assessment – Principles andframework.
Core rules for the product category of construction products.
ISO 14044
EN 16757
ISO 14044:2006: Environmental management – Life cycle
6 Environmental Product Declaration - PROMAT - Monolux®
assessment – Requirements and guidelines
Industry 2.0
ISO 45001
Industry 2.0 (from PlasticsEurope, worldsteel and ERASM).
ISO 45001:2018:Occupational health and safety management LCA database as integrated in SimaPro 9.3.0.3.
systems Requirements with guidance for use
Ordinance on Biocide Products No. 528/2012
Further references
Biocidal Products Regulation (BPR, Regulation (EU) 528/2012)
CPR
PEFCR
European Regulation N° 305/2011 (CPR)
European commission (2018). Product Environmental Footprint
Declaration of Performance Category Rules PEFCR Guidance, version 6.3.
DoP No. 0432-CPR-00541-01 - 2020/5 - Promatect®-L300 PCR Part A
ECHA candidate list Calculation rules for the Life Cycle Assessment and
Requirements on the Background Report, Institut Bauen und
Candidate List of substances of very high concern (SVHCs) for Umwelt e.V., www.bauumwelt.com.
authorisation, last update 26.07.2022, European Chemicals
Agency (ECHA), Helsinki, Finland PCR Part B
Ecoinvent Institut Bauen und Umwelt e.V, Berlin (pub.): PCR Guidance-
Texts for Building-Related Products and Services From the
Wernet, G., Bauer, C., Steubing, B., Reinhard, J., Moreno-Ruiz, range of Environmental Product Declarations of Institute
E., and Weidema, B., 2016. The ecoinvent database version 3 Construction and Environment e.V. (IBU) : Requirements on the
(part I): overview and methodology. The International Journal of EPD for Calcium silicate insulating materials
Life Cycle Assessment, [online] 21(9), pp.1218–1230. Available
at:http://link.springer.com/10.1007/s11367-016-1087-8. Pré Consultants (2021)
SimaPro 9.2.0.1 [Computer Software]. Amersfoort, The
Enperas Netherlands.
Quadrant tool. 2023. Genk, Belgium REACH
European Waste Code Regulation (EC) No 1907/2006 of the European Parliament and
of the Council of 18 December 2006 concerning the
Commission of the European Communities, 2010, Guidance on Registration, Evaluation, Authorisation and Restriction of
classification of waste according to EWC-Stat categories Chemicals (REACH), June 2017
IBU
The literature referred to in the Environmental Product
IBU 2021. Institut Bauen und Umwelt e.V.: General Instructions Declaration must be listed in full.Standards already fully quoted
for the EPD programme of Institut Bauen und Umwelt e.V., in the EPD do not need to be listed here again.
Version 2.0, Berlin: Institut Bauen und Umwelt e.V., 2021 The current version of PCR Part A and PCR Part B of the PCR
www.ibu-epd.com document on which they are based must be referenced.
7 Environmental Product Declaration - PROMAT - Monolux®
Publisher
Institut Bauen und Umwelt e.V. +49 (0)30 3087748- 0
Hegelplatz 1 info@ibu-epd.com
10117 Berlin www.ibu-epd.com
Germany
Programme holder
Institut Bauen und Umwelt e.V. +49 (0)30 3087748- 0
Hegelplatz 1 info@ibu-epd.com
10117 Berlin www.ibu-epd.com
Germany
Author of the Life Cycle Assessment
Enperas +32 3 376 00 19
Thorpark 8300 info@enperas.com
3600 Genk https://www.enperas.com/en/
Belgium
Owner of the Declaration
Etex Building Performance International +32 2 778 12 11
Rue Marcel Demonque 500 info@etexgroup.com
84915 Avignon Cedex 9 www.etexgroup.com
France
8 Environmental Product Declaration - PROMAT - Monolux®
