ENVIRONMENTAL PRODUCT DECLARATION
as per ISO 14025 and EN 15804+A2
Owner of the Declaration dormakaba International Holding GmbH
Publisher Institut Bauen und Umwelt e.V. (IBU)
Programme holder Institut Bauen und Umwelt e.V. (IBU)
Declaration number EPD-DOR-20240050-CBA1-EN
Issue date 22/03/2024
Valid to 21/03/2029
Mortise Lock Saflok RT Plus
dormakaba
www.ibu-epd.com | https://epd-online.com
General Information
dormakaba Mortise Lock Saflok RT Plus
Programme holder Owner of the declaration
IBU – Institut Bauen und Umwelt e.V. dormakaba International Holding GmbH
Hegelplatz 1 DORMA Platz 1
10117 Berlin 58256 Ennepetal
Germany Germany
Declaration number Declared product / declared unit
EPD-DOR-20240050-CBA1-EN 1 piece of the product: Saflok RT Plus consisting of the following items:
• Mortise Lock Saflok RT Plus
• lever handle
• fixing materials
• product packaging
This declaration is based on the product category rules: Scope:
Electronic and physical Access Control Systems, 01/08/2021 This Environmental Product Declaration refers to a specific mortise lock
(PCR checked and approved by the SVR) manufactured by dormakaba. The EPD is representative for the complete
Saflok RT Plus Series. The production site is located in Montreal (Canada).
Issue date Data represents the year 2024.
22/03/2024
The owner of the declaration shall be liable for the underlying information
and evidence; the IBU shall not be liable with respect to manufacturer
information, life cycle assessment data and evidences.
Valid to
21/03/2029 The EPD was created according to the specifications of EN 15804+A2. In
the following, the standard will be simplified as EN 15804.
Verification
The standard EN 15804 serves as the core PCR
Independent verification of the declaration and data according to ISO
14025:2011
internally X externally
Dipl.-Ing. Hans Peters
(Chairman of Institut Bauen und Umwelt e.V.)
Florian Pronold Matthias Klingler,
(Managing Director Institut Bauen und Umwelt e.V.) (Independent verifier)
1 Environmental Product Declaration - dormakaba - Mortise Lock Saflok RT Plus
Product
Performance data of the product with respect to its
Product description/Product definition characteristics in accordance with the relevant technical
dormakaba's RT Plus is an enhanced version of the proven RT provision which can be applied are mentioned above.
Radio-Frequency Identification (RFID) electronic lock, offering
the BLE technology directly integrated in the reader. Ideal for Base materials/Ancillary materials
retrofit, this durable lock is easy to use and works with The major material composition including the packaging of the
Ambiance and System 6000, access management software. product is listed below:
RT Plus is an easy path to RFID for properties wishing to Name Value Unit
upgrade: The switch is as simple as replacing the outside
Steel 44,5 %
housing while keeping the same door preparation.
Zinc 39,5 %
For the use and application of the product, the representative
national provisions apply. For the Saflok RT Plus Series, the Paper 7 %
standards which can be applied are the following: Stainless Steel 4,5 %
Electronics 2,5 %
• ANSI A156.13
Plastics 2 %
• ANSI A156.25
• UL 10C The product includes partial articles which contain substances
• ULC S-104 listed in the Candidate List of REACH Regulation
• EN 12209 1907/2006/EC (date: 23.01.2024) exceeding 0.1 percentage by
• EN 1634-1 mass: no
• EN 1363-1
The Candidate List can be found on the ECHA website:
Application https:echa.europa.eu/de/home
The mortise lock Saflok RT Plus is suitable for small to very
large-scale hotels. Existing mechanical or electronic door locks Reference service life
throughout a facility can be easily replaced. The access control The reference service life for the Saflok RT Plus Series
solution is ideal for guest rooms, common areas as well as amounts to 10 years, depending on the application and
back-of-houses. The BLE RFID technology enables easy frequency of use. For repairs and renewals, suitable spare
upgrade possibilities. parts are available.
The mortise lock series is tested and certified to Builders
Technical Data Hardware Manufacturers Association (BHMA) A156.13,
The Saflok RT Plus Mortise Lock series has following technical meaning they are designed to withstand a minimum of
properties: 1.000.000 cycles.
Name Value Unit
Handling left/right reversible
Door Thickness max. 66 mm
Standard Backset 70 mm
Batteries 3 AA
Mobile Access BLE enabled
Audit memory 4000 events
LCA: Calculation rules
assembly including provision of all materials, products and
Declared Unit energy, as well as waste processing up to the end-of-waste
state.
The declared unit is 1 piece of the product: Saflok RT Plus
including packaging Construction stage - Modules A4-A5
Name Value Unit The construction process stage includes:
— A4, transport to the building site; — A5, installation into the
Declared unit 1 piece/product
building; including provision of all materials, products and
Mass of declared Product 4.17 kg
energy, as well as waste processing up to the end-of-waste
state or disposal of final residues during the construction
process stage.
System boundary
System boundary Maintenance – Module B2
The type of EPD is: cradle to gate with options, modules C1– This module includes the production and the end of life of the
C4, and module D (A1–A3 + B2 + C + D and additional batteries. The potential use of batteries is declared in module
modules: A4+ A5) B2.
Production - Module A1-A3 End-of-life stage– Modules C1-C4 and D
The product stage includes: — A1, raw material extraction, The end-of-life stage includes: — C1, de-construction,
processing and mechanical treatments, processing of demolition: — C2, transport to waste processing; — C3, waste
secondary material input (e.g. recycling processes), — A2, processing for reuse, recovery and/or recycling; — C4,
transport to the manufacturer, — A3, manufacturing and disposal; including provision and all transport, provision of all
2 Environmental Product Declaration - dormakaba - Mortise Lock Saflok RT Plus
materials, products and related energy and water use. Module
D (Benefits and loads beyond the system boundary) includes: Comparability
— D, recycling potentials, expressed as net impacts and Basically, a comparison or an evaluation of EPD data is only
benefits. possible if all the data sets to be compared were created
according to EN 15804 and the building context, respectively
Geographic Representativeness the product-specific characteristics of performance, are taken
Land or region, in which the declared product system is into account. Background database: GaBi, SP40.
manufactured, used or handled at the end of the product´s
lifespan: Global
LCA: Scenarios and additional technical information
the product, the only energy consumption comes from the
Characteristic product properties of biogenic carbon battery use. The battery must be exchanged on average 5
times over the declared service life. In order to allow scaling,
Information on describing the biogenic carbon content at the exchange of 1 battery is declared in the LCA.
factory gate
Name ValueUnit
Reference service life
Biogenic carbon content in accompanying kg
0.11
packaging C Name Value Unit
Life Span according to the manufacturer 10 a
Note: 1 kg of biogenic carbon is equivalent to 44/12 kg of CO
2
End of life (C1-C4)
C1: The product dismantling from the building is done manually
without environmental burden.
C2: Transport to waste management is 50 km.
Transport to the building site (A4)
Name Value Unit
Name Value Unit Collected separately waste type waste type 3.87 kg
Litres of fuel 0.00276 l/100km Recycling 3.73 kg
Transport distance 100 km Energy recovery 0.0565 kg
Capacity utilisation (including empty runs) 55 % Landfilling 0.0916 kg
The product is transported via truck. The product is stored in The product is disassembled in a recycling process. Material
the dormakaba logistic centre in Montreal. The main distribution recycling is then assumed for metals and electronics. The
region is North America. In order to allow scaling to a specific plastic components are assumed to be incinerated with energy
point of installation 100 km are declared. recovery. The batteries and minor proportions of residues
arising from the recycling process are landfilled. Region for the
Installation into the building (A5) End of Life is: Europe.
(Depending on product)
Name Value Unit
Waste packaging (paper and plastic) 0,295 kg
Reuse, recovery and/or recycling potentials (D), relevant
Maintenance (B2) scenario information
Name Value Unit Name Value Unit
Use of batteries 5 pieces Recycling 100 %
dormakaba Mortise Lock Saflok RT Plus series are operated The collection rate is 100 %.
using a battery and are not connected to mains electricity. The
batteries are provided by dormakaba. During the operation of
3 Environmental Product Declaration - dormakaba - Mortise Lock Saflok RT Plus
LCA: Results
DESCRIPTION OF THE SYSTEM BOUNDARY (X = INCLUDED IN LCA; MND = MODULE OR INDICATOR NOT DECLARED; MNR
= MODULE NOT RELEVANT)
Benefits and
Construction loads beyond
Product stage Use stage End of life stage
process stage the system
boundaries
la ire ta m w a Ry lp p u s tro p s n a rT g n iru tc a fu n a M e h t m o rf tro p s n a rTe tis e h t o t e ta g y lb m e s s A e s U e c n a n e tn ia M ria p e R tn e m e c a lp e R tn e m h s ib ru fe R y g re n e la n o ita re p Oe s u re ta w la n o ita re p Oe s u n o itc u rts n o c -e Dn o itilo m e d tro p s n a rT g n is s e c o rp e ts a W la s o p s iD -e s u e R-y re v o c e R-g n ilc y c e Rla itn e to p
A1 A2 A3 A4 A5 B1 B2 B3 B4 B5 B6 B7 C1 C2 C3 C4 D
X X X X X MND X MNR MNR MNR MND MND X X X X X
RESULTS OF THE LCA - ENVIRONMENTAL IMPACT according to EN 15804+A2: 1 piece Saflok RT Plus
Parameter Unit A1-A3 A4 A5 B2 C1 C2 C3 C4 D
GWP-total kg CO 2 eq 3.22E+02 3.6E-02 4.22E-01 2.09E-01 0 3.8E-02 2.21E-01 1E-03 -1.8E+01
GWP-fossil kg CO 2 eq 3.2E+02 3.5E-02 1.4E-02 2.09E-01 0 3.7E-02 2.2E-01 1E-03 -1.8E+01
GWP-biogenic kg CO 2 eq 1.56E+00 2E-03 4.08E-01 2.88E-04 0 2E-03 8.18E-04 4.75E-06 2.4E-02
GWP-luluc kg CO 2 eq 4.38E-01 8.3E-07 7.08E-06 8.67E-05 0 8.73E-07 1.24E-05 4E-06 -2.7E-02
ODP kg CFC11 eq 3.4E-08 3.68E-18 7.72E-17 7.19E-16 0 3.87E-18 1.11E-16 5.15E-18 -6.99E-14
AP mol H+ eq 1.88E+00 3.49E-05 1.18E-04 2.11E-03 0 3.67E-05 3.93E-05 9.97E-06 -2.63E-01
EP-freshwater kg P eq 2.01E-03 7.46E-09 1.5E-08 1.48E-07 0 7.85E-09 1.77E-08 2.39E-09 -2.47E-05
EP-marine kg N eq 3.23E-01 1.11E-05 4.25E-05 2.54E-04 0 1.17E-05 8.86E-06 2.57E-06 -2E-02
EP-terrestrial mol N eq 3.44E+00 1.23E-04 5.31E-04 2.32E-03 0 1.3E-04 1.79E-04 2.82E-05 -2.17E-01
kg NMVOC
POCP 9.43E-01 3.14E-05 1.13E-04 7.85E-04 0 3.3E-05 2.45E-05 7.77E-06 -6.9E-02
eq
ADPE kg Sb eq 7.71E-02 1.05E-09 1.22E-09 9.05E-06 0 1.1E-09 1.52E-09 1.25E-10 -1.3E-02
ADPF MJ 3.74E+03 4.94E-01 1.34E-01 2.37E+00 0 5.2E-01 1.02E-01 1.8E-02 -2.15E+02
m3 world eq
WDP 7.97E+01 6.83E-05 5.2E-02 2.3E-02 0 7.19E-05 2.3E-02 1.46E-04 -7.72E+00
deprived
GWP = Global warming potential; ODP = Depletion potential of the stratospheric ozone layer; AP = Acidification potential of land and water; EP =
Eutrophication potential; POCP = Formation potential of tropospheric ozone photochemical oxidants; ADPE = Abiotic depletion potential for non-fossil
resources; ADPF = Abiotic depletion potential for fossil resources; WDP = Water (user) deprivation potential)
RESULTS OF THE LCA - INDICATORS TO DESCRIBE RESOURCE USE according to EN 15804+A2: 1 piece Saflok RT Plus
Parameter Unit A1-A3 A4 A5 B2 C1 C2 C3 C4 D
PERE MJ 6.72E+02 2E-03 3.57E+00 1.97E-01 0 2E-03 3.2E-02 2E-03 -3.31E+01
PERM MJ 3.55E+00 0 -3.54E+00 0 0 0 -5E-03 0 0
PERT MJ 6.75E+02 2E-03 2.4E-02 1.97E-01 0 2E-03 2.7E-02 2E-03 -3.31E+01
PENRE MJ 3.71E+03 4.95E-01 1.92E-01 2.37E+00 0 5.21E-01 3.46E+01 1.8E-02 -2.15E+02
PENRM MJ 3.46E+01 0 -5.9E-02 0 0 0 -3.45E+01 0 0
PENRT MJ 3.74E+03 4.95E-01 1.34E-01 2.37E+00 0 5.21E-01 1.02E-01 1.8E-02 -2.15E+02
SM kg 2.15E+00 0 0 0 0 0 0 0 0
RSF MJ 0 0 0 0 0 0 0 0 0
NRSF MJ 0 0 0 0 0 0 0 0 0
FW m3 2.02E+00 2.8E-06 1E-03 7.23E-04 0 2.94E-06 5.4E-04 4.6E-06 -1.56E-01
PERE = Use of renewable primary energy excluding renewable primary energy resources used as raw materials; PERM = Use of renewable primary
energy resources used as raw materials; PERT = Total use of renewable primary energy resources; PENRE = Use of non-renewable primary energy
excluding non-renewable primary energy resources used as raw materials; PENRM = Use of non-renewable primary energy resources used as raw
materials; PENRT = Total use of non-renewable primary energy resources; SM = Use of secondary material; RSF = Use of renewable secondary fuels;
NRSF = Use of non-renewable secondary fuels; FW = Use of net fresh water
RESULTS OF THE LCA – WASTE CATEGORIES AND OUTPUT FLOWS according to EN 15804+A2:
1 piece Saflok RT Plus
Parameter Unit A1-A3 A4 A5 B2 C1 C2 C3 C4 D
HWD kg 2.75E-04 4.8E-11 2.01E-10 1.15E-08 0 5.05E-11 3.89E-10 2.78E-10 -2.66E-06
NHWD kg 1.16E+01 5.06E-05 1.3E-02 1E+00 0 5.33E-05 2.3E-02 9.2E-02 -2.9E+00
RWD kg 9.8E-02 5.31E-07 7.01E-06 4.87E-05 0 5.59E-07 3.79E-06 2.08E-07 -4E-03
CRU kg 0 0 0 0 0 0 0 0 0
MFR kg 0 0 0 0 0 0 8.6E+00 0 0
MER kg 0 0 0 0 0 0 0 0 0
EEE MJ 0 0 6.4E-01 0 0 0 3.52E+00 0 0
EET MJ 0 0 1.16E+00 0 0 0 8.17E+00 0 0
4 Environmental Product Declaration - dormakaba - Mortise Lock Saflok RT Plus
HWD = Hazardous waste disposed; NHWD = Non-hazardous waste disposed; RWD = Radioactive waste disposed; CRU = Components for re-use;
MFR = Materials for recycling; MER = Materials for energy recovery; EEE = Exported electrical energy; EET = Exported thermal energy
RESULTS OF THE LCA – additional impact categories according to EN 15804+A2-optional:
1 piece Saflok RT Plus
Parameter Unit A1-A3 A4 A5 B2 C1 C2 C3 C4 D
Disease
PM 1.91E-05 1.83E-10 6.57E-10 1.52E-08 0 1.93E-10 5E-10 1.23E-10 -2.28E-06
incidence
IR kBq U235 eq 9.64E+00 7.59E-05 1E-03 5.24E-03 0 7.99E-05 3.42E-04 2.14E-05 -3.54E-01
ETP-fw CTUe 1.79E+03 3.5E-01 6.3E-02 6.06E-01 0 3.69E-01 3.8E-02 1E-02 -1.36E+02
HTP-c CTUh 3.3E-07 6.59E-12 3.37E-12 5.97E-11 0 6.94E-12 3.32E-12 1.54E-12 1.25E-08
HTP-nc CTUh 6.58E-06 2.82E-10 1.49E-10 3.41E-09 0 2.97E-10 3.35E-10 1.7E-10 1.84E-06
SQP SQP 6.34E+02 1E-03 3.6E-02 4.61E-01 0 1E-03 3.1E-02 4E-03 -1.04E+02
PM = Potential incidence of disease due to PM emissions; IR = Potential Human exposure efficiency relative to U235; ETP-fw = Potential comparative
Toxic Unit for ecosystems; HTP-c = Potential comparative Toxic Unit for humans (cancerogenic); HTP-nc = Potential comparative Toxic Unit for humans
(not cancerogenic); SQP = Potential soil quality index
Disclaimer 1 – for the indicator “Potential Human exposure efficiency relative to U235”. This impact category deals mainly with the
eventual impact of low-dose ionizing radiation on human health of the nuclear fuel cycle. It does not consider effects due to possible
nuclear accidents, occupational exposure or radioactive waste disposal in underground facilities. Potential ionizing radiation from the
soil, radon and from some construction materials is also not measured by this indicator.
Disclaimer 2 – for the indicators “abiotic depletion potential for non-fossil resources”, “abiotic depletion potential for fossil resources”,
“water (user) deprivation potential, deprivation-weighted water consumption”, “potential comparative toxic unit for ecosystems”,
“potential comparative toxic unit for humans – cancerogenic”, “Potential comparative toxic unit for humans - not cancerogenic”,
“potential soil quality index”. The results of this environmental impact indicator shall be used with care as the uncertainties on these
results are high as there is limited experience with the indicator.
This EPD was created using a software tool.
References
ANSI A156.25:2023 Regulation (EC) No 1907/2006 of the European Parliament and
ANSI A156.25:2023, Electrified Locking Devices of the Council on the Registration, Evaluation, Authorisation
and Restriction of Chemicals (REACH)
ANSI A156.13:2022
ANSI A156.13:2022, Mortise Locks RoHS
2011/65/EU, Directive on the restriction of the use of certain
BHMA hazardous substances in electrical and electronic equipment
Builders Hardware Manufacturers Association
UL 10C:2016
ECHA UL 10C:2016-06, Standard for Safety Positive Pressure Fire
European Chemicals Agency Tests of Door Assemblies
EN 12209:2016 ULC CAN-S104:2020
EN 12209:2016, Building hardware - Mechanically operated ULC CAN-S104:2020-08, Standard Method for Fire Tests of
locks and locking plates - Requirements and test methods Door Assemblies
EN 1634-1:2018 Further References
EN 1634-1:2018-04, Fire resistance and smoke control tests for
door and shutter assemblies, openable windows and elements GaBi
of building hardware Sphera Solutions GmbH
Gabi Software System and Database for Life Cycle Engineering
EN 1363-1:2020-05 19922020
EN 1363-1:2020-05, Fire resistance tests - Part 1: General Version 10.0.0.71
requirements University of Stuttgart
Leinfelden-Echterdingen
EN 15804
EN 15804+A2:2019+AC:2021, Sustainability of construction GaBi ts documentation
works — Environmental Product Declarations — Core rules for GaBi life cycle inventory data documentation
the product category of construction products (https://www.gabisoftware.com/support/gabi/gabidatabase-
2020-lcidocumentation/).
ISO 14025
ISO 14025:201110, Environmental labels and declarations — IBU 2021
Type III environmental declarations — Principles and General Instructions for the EPD programme
procedures of Institut Bauen und Umwelt e.V. Version 2.0, Berlin: Institut
Bauen und Umwelt e.V., 2021. www.ibu-epd.com
RFID
Radio-Frequency Identification LCA-tool dormakaba
Tool No.: IBU-DOR-202109-LT1-EN.
REACH Developed by Sphera Solutions GmbH
5 Environmental Product Declaration - dormakaba - Mortise Lock Saflok RT Plus
PCR Part B
PCR Part A PCR – Part B: Requirements on the EPD for Electronic and
PCR – Part A: Calculation Rules for the Life Cycle Assessment physical Access Control Systems, version 08/2021, Institut
and Requirements on the Project Re-port according to EN Bauen und Umwelt e.V., www.ibu-epd.com.
15804+A2:2019, Version 1.0, 2020, Institut Bauen und Umwelt
e.V., www.ibu-epd.com.
6 Environmental Product Declaration - dormakaba - Mortise Lock Saflok RT Plus
Publisher
Institut Bauen und Umwelt e.V. +49 (0)30 3087748- 0
Hegelplatz 1 info@ibu-epd.com
10117 Berlin www.ibu-epd.com
Germany
Programme holder
Institut Bauen und Umwelt e.V. +49 (0)30 3087748- 0
Hegelplatz 1 info@ibu-epd.com
10117 Berlin www.ibu-epd.com
Germany
Author of the Life Cycle Assessment
dormakaba International Holding GmbH +49 2333 793-0
DORMA Platz 1 info.de@dormakaba.com
58256 Ennepetal www.dormakaba.com
Germany
Owner of the Declaration
dormakaba International Holding GmbH +49 2333 793-0
DORMA Platz 1 info.de@dormakaba.com
58256 Ennepetal www.dormakaba.com
Germany
7 Environmental Product Declaration - dormakaba - Mortise Lock Saflok RT Plus
