Environmental product declaration
In accordance with ISO 14025 and EN15804+A2
NC bolt M33 with spherical plate Pc-Coat®
Owner of the declaration: Program operator:
Pretec Norge AS The Norwegian EPD Foundation
Product: Declaration number:
NC bolt M33 with spherical plate Pc-Coat® NEPD-8849-8512
Declared unit: Registration number:
1 kg NEPD-8849-8512
This declaration is based on Product Category Rules: Issue date:
CEN Standard EN 15804:2012+A2:2019 serves as core 29.01.2025
PCR
Valid to:
The Norwegian EPD Foundation NPCR 013:2021 Part B for Steel and aluminium 29.01.2030
construction products
EPD software:
LCAno EPD generator ID: 578679
1 / 12
General information
Product Owner of the declaration:
NC bolt M33 with spherical plate Pc-Coat® Pretec Norge AS
Contact person: Ernad Sarajlija
Phone: (+47 69 10 24 60
e-mail: post@pretec.no
Program operator: Manufacturer:
The Norwegian EPD Foundation Pretec Norge AS
Post Box 5250 Majorstuen, 0303 Oslo, Norway Kampenesmosen 3
Phone: +47 977 22 020 1739 Borgenhaugen, Norway
web: www.epd-norge.no
Declaration number: Place of production:
NEPD-8849-8512 Pretec China
Zhejiang Pretec Metal Products Co., Ltd. Nr.9, Jinchang Rd, Haining
Zhejiang Province, P.R:, China
This declaration is based on Product Category Rules: Management system:
CEN Standard EN 15804:2012+A2:2019 serves as core PCR ISO 14001, ISO 9001 and ISO45001, AAA Sertification AB, sert no
NPCR 013:2021 Part B for Steel and aluminium construction products 794 - EN 1090-1, AAA Sertification AB, sert no 2296
Statement of liability: Organisation no:
The owner of the declaration shall be liable for the underlying NO 980 429 245 MVA
information and evidence. EPD Norway shall not be liable with respect
to manufacturer information, life cycle assessment data and
evidences.​
Declared unit: Issue date:
1 kg NC bolt M33 with spherical plate Pc-Coat® 29.01.2025
Declared unit with option: Valid to:
A1-A3,A4,A5,C1,C2,C3,C4,D 29.01.2030
Year of study:
2024
Functional unit: Comparability:
1kg of NC bolt M33x4000 including expansion shell and spherical EPD of construction products may not be comparable if they not
plate. comply with EN 15804 and seen in a building context.
NB! For other lengths see variants table at the end of the document.
General information on verification of EPD from EPD tools: Development and verification of EPD:
Independent verification of data, other environmental information The declaration is created using EPD tool lca.tools NEPDT038,
and the declaration according to ISO 14025:2010, § 8.1.3 and § 8.1.4. developed by LCA.no. The EPD tool is integrated in the company's
Verification of each EPD is made according to EPD-Norway’s management system, and has been approved by EPD Norway.
guidelines for verification and approval requiring that tools are i)
integrated into the company's environmental management system, ii) Developer of EPD: Christine B.-Norén
the procedures for use of the EPD tool are approved by EPD-Norway,
Reviewer of company-specific input data and EPD:​ Ernad Sarajlija
and iii) the process is reviewed annually by an independent third
party verifier. See Appendix G of EPD-Norway's General Programme
Instructions for further information on EPD tools
Verification of EPD tool: Approved:
Independent third party verification of the EPD tool, background data
and test-EPD in accordance with EPDNorway's procedures and
guidelines for verification and approval of EPD tools.
Third party verifier:
Alexander Borg, Asplan Viak AS
(no signature required)
2 / 12
Product
Product description:
A NC-Bolt is a combination bolt that is installed for immediate support of rock in tunnels or slopes. It is immediately anchored when installed by
an expansion shell providing work safety and can be fully grouted at a later stage, allowing it to be classified as permanent support. NC-Bolt with
PC-coat provides market leading service life in the most demanding environments.
Product specification
The NC-bolt is a rebar-based combination bolt made from scrap/recycled steel material. It has a grouting system made of a steel head and a
special designed plastic tube to ensure perfect grouting and full anchoring capacity.
All steel parts except the expansion shell (it has only a temporarily function) has Pc-Coat® as the standard corrosion protection. Pc-Coat® is a
duplex coating system providing the optimal corrosion protection to ensure long service life in all conditions. Pc-Coat™ is suitable for use in all
atmospheric corrosion classes, included CX, according to EN ISO 12944-2:2017.
This EPD is based on complete bolt with all accessories and spherical plate.
Materials kg %
Plastic - Polypropylene (PP) 0,03 3,31
Powder coating 0,00 0,20
Metal - Steel 0,95 95,49
Metal - Zinc 0,01 1,00
Total 1,00 100,00
Packaging kg %
Packaging - Pallet 0,02 93,75
Packaging - Plastic 0,00 6,25
Total incl. packaging 1,01 100,00
Technical data:
- Bolt material: High-ductility rebar B500NC acc. NS 3576-1:2024
- Thread length: 2xM20x150mm (cold rolled thread).
- Mechanical properties: Tension area 245/314 mm2 (thread/stem), Yield Strength: (ReH) 500 N/mm2, Tensile Strength: (Rm) 600 N/mm2,
Ductility: AGT min 8 %
- Corrosion protection: Pc-Coat®: Hot-dip galvanizing acc. ISO 1461 + Zinc-manganese phosphating + Powder coating according to EN 13438.
Tested and approved for all corrosion classes, included CX, according to EN ISO 12944-2:2017.
- CE-marked acc. EN 1090
Market:
worldwide
Reference service life, product
120 years
Reference service life, building or construction works
LCA: Calculation rules
Declared unit:
1 kg NC bolt M33 with spherical plate Pc-Coat®
Cut-off criteria:
All major raw materials and all the essential energy is included. The production processes for raw materials and energy flows with very small
amounts (less than 1%) are not included. These cut-off criteria do not​ apply for hazardous materials and substances.
Allocation:
The allocation is made in accordance with the provisions of EN 15804. Incoming energy and water and waste production in-house is allocated
equally among all products through mass allocation. Effects of primary production of recycled materials is allocated to the main product in which
the material was used. The recycling process and transportation of the material is allocated to this analysis.
Data quality:
Specific data for the product composition are provided by the manufacturer. The data represent the production of the declared product and were
collected for EPD development in the year of study. Background data is based on EPDs according to EN 15804 and different LCA databases. The
data quality of the raw materials in A1 is presented in the table below.
3 / 12
Materials Source Data quality Year
Metal - Steel ecoinvent 3.6 Database 2019
Metal - Steel Modified ecoinvent 3.6 Database 2019
Metal - Zinc ecoinvent 3.6 Database 2019
Plastic - Polypropylene (PP) ecoinvent 3.6 Database 2019
Packaging - Pallet Modified ecoinvent 3.6 Database 2019
Packaging - Plastic ecoinvent 3.6 Database 2019
Powder coating Ecoinvent 3.6 Database 2019
4 / 12
System boundaries (X=included, MND=module not declared, MNR=module not relevant)
Construction Beyond the system
Product stage Use stage End of life stage
installation stage boundaries
A1 A2 A3 A4 A5 B1 B2 B3 B4 B5 B6 B7 C1 C2 C3 C4 D
X X X X X MND MND MND MND MND MND MND X X X X X
System boundary:
This EPD is a “cradle-to-gate with options” EPD. The system boundary for this LCA report is from A1 to A5, C1-C4 and D
Additional technical information:
Bolts are delivered with pre-assembled expansion shells and packages are suited for stacking to optimize logistics.
waR slairetam tropsnarT gnirutcafunaM tropsnarT ylbmessA e​sU ecnanetniaM riapeR tnemecalpeR tnemhsibrufeR lanoitarepO ygrene esu lanoitarepO esu retaw -eD noitcurtsnoc noitilomed tropsnarT etsaW gnissecorp lasopsiD -yrevoceR-esueR laitnetop-gnilcyceR
5 / 12
LCA: Scenarios and additional technical information
The following information describe the scenarios in the different modules of the EPD.
Module C "End of life stage" is a generic scenario for decommissioning of construction. Subject to project specific conditions. Grade of recycling for
different
steel grades is based on statistics obtained from Norsk Stålforbund.
Capacity utilisation Value
Transport from production place to user (A4) Distance (km) Fuel/Energy Consumption Unit
(incl. return) % (Liter/tonne)
Truck, 16-32 tonnes, EURO 6 (km) 36,7 % 300 0,043 l/tkm 12,90
Assembly (A5) Unit Value
Diesel, burned (L) L/DU 0,00010
Waste, wood, average treatment - A5, inkl. transp.
kg/DU 0,010
(kg)
Waste, packaging, pallet, EUR wooden pallet,
reusable, average treatment (kg) - A5, inkl. 85 km kg 0,015
transp.
Waste, packaging, plastic film (LDPE), to average
kg 0,0010
treatment (kg) - A5, inkl. 85 km transp.
De-construction demolition (C1) Unit Value
Diesel, burned (MJ) MJ/DU 0,62
Waste processing (C3) Unit Value
Waste treatment per kg Hazardous waste,
kg 0,0020
incineration (kg) - C3
Materials to recycling (kg) kg 0,85
Waste treatment per kg Polypropylene (PP),
kg 0,033
incineration with fly ash extraction (kg) - C3
Disposal (C4) Unit Value
Landfilling of ashes from incineration of
kg 0,00037
Hazardous waste, from incineration (kg) - C4
Waste, scrap steel, to landfill (kg) kg 0,10
Landfilling of ashes from incineration of
Polypropylene (PP), process per kg ashes and kg 0,00098
residues (kg) - CH - C4
Benefits and loads beyond the system
Unit Value
boundaries (D)
Substitution of electricity, in Norway (MJ) MJ 0,053
Substitution of thermal energy, district heating, in
MJ 0,81
Norway (MJ)
Substitution of Zinc (kg) kg 0,0085
Substitution of primary steel with net scrap (kg) kg -0,023
6 / 12
LCA: Results
The LCA results are presented below for the declared unit defined on page 2 of the EPD document.
Environmental impact
Indicator Unit A1-A3 A4 A5 C1 C2 C3 C4 D
GWP-total kg CO2 -eq 1,01E+00 4,90E-02 2,35E-02 5,73E-02 4,90E-02 8,85E-02 6,82E-04 -5,38E-03
GWP-fossil kg CO2 -eq 1,03E+00 4,90E-02 7,22E-04 5,73E-02 4,90E-02 8,85E-02 6,81E-04 -4,90E-03
GWP-biogenic kg CO2 -eq -2,05E-02 2,03E-05 2,27E-02 1,07E-05 2,03E-05 1,18E-05 4,87E-07 -2,44E-04
GWP-luluc kg CO2 -eq 1,21E-03 1,74E-05 1,08E-07 4,52E-06 1,74E-05 1,23E-06 1,15E-07 -2,36E-04
ODP kg CFC11 -eq 7,19E-08 1,11E-08 1,27E-10 1,24E-08 1,11E-08 5,74E-10 2,38E-10 -3,43E-04
AP mol H+ -eq 5,61E-03 1,41E-04 6,12E-06 6,00E-04 1,41E-04 1,71E-05 5,02E-06 -1,66E-04
EP-FreshWater kg P -eq 4,67E-05 3,92E-07 4,92E-09 2,09E-07 3,92E-07 1,13E-07 5,79E-09 -1,80E-06
EP-Marine kg N -eq 1,20E-03 2,79E-05 2,72E-06 2,65E-04 2,79E-05 6,42E-06 1,83E-06 -4,25E-05
EP-Terrestial mol N -eq 1,23E-02 3,12E-04 2,89E-05 2,90E-03 3,12E-04 7,00E-05 2,03E-05 -4,99E-04
POCP kg NMVOC -eq 4,81E-03 1,19E-04 7,79E-06 7,98E-04 1,19E-04 1,74E-05 5,79E-06 -6,82E-05
ADP-minerals&metals1 kg Sb-eq 8,03E-04 1,35E-06 5,66E-09 8,80E-08 1,35E-06 1,86E-08 4,66E-09 -6,59E-04
ADP-fossil1 MJ 1,39E+01 7,41E-01 8,59E-03 7,89E-01 7,41E-01 2,43E-02 1,61E-02 -2,33E-01
WDP1 m3 1,30E+01 7,17E-01 7,42E-03 1,68E-01 7,17E-01 8,21E-02 5,63E-02 -3,12E+00
GWP-total = Global Warming Potential total; GWP-fossil = Global Warming Potential fossil fuels; GWP-biogenic = Global Warming Potential biogenic; GWP-luluc =
Global Warming Potential land use and land use change; ODP = Depletion potential of the stratospheric ozone layer; AP = Acidification potential, Accumulated
Exceedance; EP-freshwater = Eutrophication potential, fraction of nutrients reaching freshwater end compartment: EP-marine = Eutrophication potential, fraction of
nutrients reaching marine end compartment; EP-terrestrial = Eutrophication potential, Accumulated Exceedance; POCP = Formation potential of tropospheric ozone;
ADP-minerals&metals = Abiotic depletion potential for non-fossil resources; ADP-fossil = Abiotic depletion for fossil resources potential; WDP = Water (user)
deprivation potential, deprivation-weighted water consumption
"Reading example: 9,0 E-03 = 9,0*10-3 = 0,009"
*INA Indicator Not Assessed
1. The results of this environmental impact indicator shall be used with care as the uncertainties on these results are high or as there is limited experienced with the
indicator
Remarks to environmental impacts
7 / 12
Additional environmental impact indicators
Indicator Unit A1-A3 A4 A5 C1 C2 C3 C4 D
PM Disease incidence 1,18E-07 3,00E-09 1,28E-10 1,59E-08 3,00E-09 1,50E-10 1,01E-10 -1,25E-09
IRP2 kgBq U235 -eq 3,00E-02 3,24E-03 3,46E-05 3,38E-03 3,24E-03 9,46E-05 7,13E-05 -3,32E-03
ETP-fw1 CTUe 2,97E+01 5,49E-01 6,84E-03 4,31E-01 5,49E-01 1,07E-01 1,05E-02 -2,83E-01
HTP-c1 CTUh 1,00E-08 0,00E+00 0,00E+00 1,70E-11 0,00E+00 6,00E-12 0,00E+00 -3,20E-11
HTP-nc1 CTUh 2,87E-07 6,00E-10 2,20E-11 3,96E-10 6,00E-10 9,80E-11 1,00E-11 -7,28E-09
SQP1 dimensionless 4,58E+00 5,18E-01 3,09E-03 1,00E-01 5,18E-01 8,05E-03 5,78E-02 -6,11E-01
PM = Particulate Matter emissions; IRP = Ionizing radiation – human health; ETP-fw = Eco toxicity – freshwater; HTP-c = Human toxicity – cancer effects; HTP-nc =
Human toxicity – non cancer effects; SQP = Potential Soil Quality Index (dimensionless)
"Reading example: 9,0 E-03 = 9,0*10-3 = 0,009"
*INA Indicator Not Assessed
1. The results of this environmental impact indicator shall be used with care as the uncertainties on these results are high or as there is limited experienced with the
indicator
2. This impact category deals mainly with the eventual impact of low dose ionizing radiation on human health of the nuclear fuel cycle. It does not consider effects due
to possible nuclear accidents, occupational exposure nor due to radioactive waste disposal in underground facilities. Potential ionizing radiation from the soil, from
radon and from some construction materials is also not measured by this indicator.
8 / 12
Resource use
Indicator Unit A1-A3 A4 A5 C1 C2 C3 C4 D
PERE MJ 7,11E+00 1,06E-02 1,04E-04 4,27E-03 1,06E-02 3,53E-03 3,53E-04 -4,49E-01
PERM MJ 2,08E-01 0,00E+00 -2,08E-01 0,00E+00 0,00E+00 0,00E+00 0,00E+00 0,00E+00
PERT MJ 7,31E+00 1,06E-02 -2,08E-01 4,27E-03 1,06E-02 3,53E-03 3,53E-04 -4,49E-01
PENRE MJ 1,28E+01 7,41E-01 8,59E-03 7,89E-01 7,41E-01 2,43E-02 1,61E-02 -2,33E-01
PENRM MJ 1,12E+00 0,00E+00 -4,25E-02 0,00E+00 0,00E+00 0,00E+00 0,00E+00 0,00E+00
PENRT MJ 1,39E+01 7,41E-01 -3,39E-02 7,89E-01 7,41E-01 2,43E-02 1,61E-02 -2,33E-01
SM kg 8,69E-01 0,00E+00 1,60E-06 3,87E-04 0,00E+00 0,00E+00 0,00E+00 0,00E+00
RSF MJ 1,24E-02 3,79E-04 2,90E-06 1,05E-04 3,79E-04 7,88E-05 7,18E-06 -2,37E-03
NRSF MJ 2,94E-01 1,36E-03 3,33E-05 1,54E-03 1,36E-03 0,00E+00 1,49E-04 -5,27E-02
FW m3 1,45E-02 7,92E-05 2,90E-06 4,06E-05 7,92E-05 3,30E-05 1,96E-05 -1,25E-03
PERE = Use of renewable primary energy excluding renewable primary energy resources used as raw materials; PERM = Use of renewable primary energy resources used
as raw materials; PERT = Total use of renewable primary energy resources; PENRE = Use of non renewable primary energy excluding non-renewable primary energy
resources used as raw materials; PENRM = Use of non renewable primary energy resources used as raw materials; PENRT = Total use of non renewable primary energy
resources; SM = Use of secondary materials; RSF = Use of renewable secondary fuels; NRSF = Use of non-renewable secondary fuels; FW = Net use of fresh water
"Reading example: 9,0 E-03 = 9,0*10-3 = 0,009"
*INA Indicator Not Assessed
9 / 12
End of life - Waste
Indicator Unit A1-A3 A4 A5 C1 C2 C3 C4 D
HWD kg 4,23E-03 3,82E-05 1,03E-04 2,32E-05 3,82E-05 0,00E+00 8,31E-04 -2,22E-04
NHWD kg 2,81E-01 3,60E-02 1,92E-03 9,34E-04 3,60E-02 2,00E-03 1,09E-01 5,09E-03
RWD kg 3,06E-05 5,05E-06 5,10E-08 5,48E-06 5,05E-06 0,00E+00 2,91E-09 -2,40E-06
HWD = Hazardous waste disposed; NHWD = Non-hazardous waste disposed; RWD = Radioactive waste disposed
"Reading example: 9,0 E-03 = 9,0*10-3 = 0,009"
*INA Indicator Not Assessed
End of life - Output flow
Indicator Unit A1-A3 A4 A5 C1 C2 C3 C4 D
CRU kg 0,00E+00 0,00E+00 1,43E-02 0,00E+00 0,00E+00 0,00E+00 0,00E+00 0,00E+00
MFR kg 2,33E-02 0,00E+00 5,15E-04 3,80E-04 0,00E+00 8,55E-01 0,00E+00 0,00E+00
MER kg 2,07E-05 0,00E+00 7,44E-04 1,18E-06 0,00E+00 3,50E-02 0,00E+00 0,00E+00
EEE MJ 1,38E-04 0,00E+00 7,47E-03 4,04E-06 0,00E+00 5,37E-02 0,00E+00 0,00E+00
EET MJ 2,09E-03 0,00E+00 1,13E-01 6,12E-05 0,00E+00 8,13E-01 0,00E+00 0,00E+00
CRU = Components for re-use; MFR = Materials for recycling; MER = Materials for energy recovery; EEE = Exported energy electrical; EET = Exported energy thermal
"Reading example: 9,0 E-03 = 9,0*10-3 = 0,009"
*INA Indicator Not Assessed
Biogenic Carbon Content
Indicator Unit At the factory gate
Biogenic carbon content in product kg C 0,00E+00
Biogenic carbon content in accompanying packaging kg C 6,20E-03
Note: 1 kg biogenic carbon is equivalent to 44/12 kg CO2
10 / 12
Additional requirements
Greenhouse gas emissions from the use of electricity in the manufacturing phase
National production mix from import, low voltage (production of transmission lines, in addition to direct emissions and losses in grid) of applied
electricity for the manufacturing process (A3).
Dangerous substances
The product contains no substances given by the REACH Candidate list.
Indoor environment
Additional Environmental Information
Additional environmental impact indicators required in NPCR Part A for construction products
Indicator Unit A1-A3 A4 A5 C1 C2 C3 C4 D
GWPIOBC kg CO2 -eq 1,03E+00 4,90E-02 4,53E-04 5,67E-02 4,90E-02 8,85E-02 6,84E-04 7,31E-03
GWP-IOBC: Global warming potential calculated according to the principle of instantaneous oxidation. In order to increase the transparency of biogenic carbon​
contribution to climate impact, the indicator GWP-IOBC is required as it declares climate impacts calculated according to the principle of instantaneous oxidation.​
GWP-IOBC is also referred to as GWP-GHG in context to Swedish public procurement legislation.
Variants and Options
Key environmental indicators (A1-A3) for variants of this EPD
Variants Weight (kg) GWPtotal (kg CO2 -eq) Total energy consumption (MJ) Amount of recycled materials (%)
NC bolt M33x3000 with spherical plate Pc-Coat® 1,00 1,07 20,66 84,81
NC bolt M33x4000 with spherical plate Pc-Coat® 1,00 1,01 20,19 86,94
NC bolt M33x5000 with spherical plate Pc-Coat® 1,00 0,95 19,65 88,54
NC bolt M33x6000 with spherical plate Pc-Coat® 1,00 0,96 19,96 89,64
NC bolt M33x8000 with spherical plate Pc-Coat® 1,00 0,94 19,89 91,15
Key environmental indicators (A1-A3) for options for this EPD
Options Weight (kg) GWPtotal (kg CO2 -eq) Total energy consumption (MJ) Amount of recycled materials (%)
NC bolt M33x3000 Pc-Coat® 1,00 0,95 20,07 91,48
NC bolt M33x4000 Pc-Coat® 1,00 0,92 19,81 92,46
NC bolt M33x5000 Pc-Coat® 1,00 0,92 19,88 93,26
NC bolt M33x6000 Pc-Coat® 1,00 0,90 19,75 93,55
NC bolt M33x8000 Pc-Coat® 1,00 0,88 19,62 94,24
11 / 12
Bibliography
ISO 14025:2010 Environmental labels and declarations - Type III environmental declarations - Principles and procedures.
ISO 14044:2006 Environmental management - Life cycle assessment - Requirements and guidelines.
EN 15804:2012+A2:2019 Environmental product declaration - Core rules for the product category of construction products.
ISO 21930:2017 Sustainability in buildings and civil engineering works - Core rules for environmental product declarations of construction
products.
ecoinvent v3, Allocation, cut-off by classification, Swiss Centre of Life Cycle Inventories.
Iversen et al., (2021) eEPD v2021.09 Background information for EPD generator tool system verification, LCA.no Report number: 07.21
Graafland and Iversen, (2022) EPD generator for EPD generator for NPCR 013 Part B for Steel and Aluminum, Background information for EPD
generator application and LCA data, LCA.no report number: 08.22
NPCR Part A: Construction products and services. Ver. 2.0. April 2021, EPD-Norge.
NPCR 013 Part B for Steel and Aluminium Construction Products , Ver. 4.0, 06.10.2021, EPD Norway.
Program operator and publisher Phone: +47 977 22 020
The Norwegian EPD Foundation e-mail: post@epd-norge.no
Post Box 5250 Majorstuen, 0303 Oslo, Norway web: www.epd-norge.no
Owner of the declaration: Phone: (+47) 69 10 24 60
Pretec Norge AS e-mail: post@pretec.no
Kampenesmosen 3, 1739 Borgenhaugen, Norway web: www.pretec.no
Author of the Life Cycle Assessment Phone: +47 916 50 916
LCA.no AS e-mail: post@lca.no
Dokka 6A, 1671 Kråkerøy, Norway web: www.lca.no
Developer of EPD generator Phone: +47 916 50 916
LCA.no AS e-mail: post@lca.no
Dokka 6A, 1671 Kråkerøy, Norway web: www.lca.no
ECO Platform web: www.eco-platform.org
ECO Portal web: ECO Portal
12 / 12
