Ver. 1 2015
ENVIRONMENTAL PRODUCT DECLARATION
in accordance with ISO 14025 and EN 15804+A1
Owner of the declaration: SunPower
Program operator: The Norwegian EPD Foundation
Publisher: The Norwegian EPD Foundation
Declaration and registration number: NEPD-3087-1726-EN
Issue date: 09.09.2021
Valid to: 09.09.2026
MAXEON 3 MONO-CRYSTALLINE PHOTOVOLTAIC MODULE
SunPower
www.epd-norge.no
NEPD-3087-1726-EN MAXEON 3 MONO-CRYSTALLINE PHOTOVOLTAIC MODULE
General information
Product Owner of the declaration
MAXEON 3 SunPower
MONO-CRYSTALLINE PHOTOVOLTAIC MODULE
Manufacturer
Program holder SunPower
The Norwegian EPD Foundation
12 Allée du Levant, 69890 La Tour de Salvagny, France
Post Box 5250 Majorstuen, 0303 Oslo, Norway Phone: (+33) 7 60 59 84 73
Phone: (+47) 23 08 80 00 e-mail: Karin.Alberto-Burkhardt@sunpower.com
e-mail: post@epd-norge.no Web: www.sunpower.com
Declaration number Place of production:
NEPD-3087-1726-EN Prolongación Lazaro Cardenas, Agustín Sanguines 3101, Huertas
de La Progreso, 21188 Mexicali, B.C
Mexico
This declaration is based on Product Category Rules:
NPCR 029 version 1.1
Management system:
ISO 14001, ISO 9001
Statements
The owner of the declaration shall be liable for the underlying
information and evidence.
EPD Norway shall not be liable with respect to manufacturer,
Organisation no:
life cycle assessment data and evidences.
FR52344584818
Issue date
09.09.2021
Valid to
09.09.2026
Declared unit:
1m² of mono-crystalline solar panel
Year of study:
2020
Declared unit with option:
N/A
Comparability:
EPD of construction products may not be comparable
if they do not comply with EN15804 and are seen in a
building context
Functional unit:
1 Wp of manufactured photovoltaic module, from cradle-to-
grave, with activities needed for a study period for a defined
reference service life (≥80% of the labelled power output)
The EPD has been worked out by:
Verification:
EVEA
Independent verification of the declaration and data, 11 rue Voltaire
according to ISO14025:2010 44000 NANTES
FRANCE
☐internal ☒external
Third party verifier:
Michael M. Jenssen, Asplan Viak AS
(Independent verifier approved by EPD Norway) Approved
NEPD-3087-1726-EN MAXEON 3 MONO-CRYSTALLINE PHOTOVOLTAIC MODULE
1/7
Product
Product description: Technical data:
400Wp mono-crystalline solar photovoltaic The panel considered for this EPD has a power rating of 400W.
module with back-contact conductivity, solid 1 complete panel has a mass of 19 kg without packaging.
metal backing and thick connectors. The The packaging per panel weighs 1.36 kg.
panels are designed to be installed on roofs The overall dimensions are 1690x1046x40 mm.
or as stand-alone systems for local power
production. Certified: IEC 61215, IEC 61730 Class 1 fire rated per UNI
9177
The 2 other products covered by the PEP
differ only in colour for the BLK product and Market:
the connector type for the COM product. Norway / Europe / World
As the differences between products is Reference service life:
minor, no averaging has been performed. 25 years
To produce their panels, SunPower sources
silicon wafers from Norway and the US,
which are sent to their factory in the
Phillipines to produce the solar cells. These
cells are then sent to their factory in
Mexico, where they are assembled with the
backsheet, frame and electrical connections
to produce the finished solar module.
Product specification
Sold as individual panels, with an effective
surface area of 1.77m². The packaging
consists of LDPE film, PP, PET and a
cardboard box, and the panels are
delivered on a wooden pallet.
The product consists of the following
materials per functional unit:
Materials kg / FU %
Copper 1,63E-04 0,31%
Tin 6,52E-06 0,01%
Silver 2,72E-07 0,00%
Cell 1,19E-03 2,29%
Label 1,23E-05 0,02%
Junction BOX 5,49E-04 1,06%
Backsheet PET 8,14E-04 1,57%
EVA 3,52E-03 6,80%
Aluminium 3,99E-03 7,72%
Solar glass 3,81E-02 73,58%
Packaging : LDPE
3,85E-07 0,00%
Film
Packaging : PP 4,09E-04 0,79%
Packaging : PET 8,14E-04 1,57%
Packaging :
2,56E-05 0,05%
Cardboard
Packaging : Pallet 2,17E-03 4,20%
NEPD-3087-1726-EN MAXEON 3 MONO-CRYSTALLINE PHOTOVOLTAIC MODULE
2/7
LCA: Calculation rules
Functional unit: System boundary:
1 Wp of manufactured photovoltaic module, from cradle-to-grave, The flow chart for the life cycle of SunPower Maxeon
with activities needed for a study period for a defined reference panels is shown below.
service life (≥80% of the labelled power output)
Declared unit:
1 m² of photovoltaic module – 1 m² = 226 Wp
Allocation:
The allocation is made in accordance with the provisions of ISO
Data quality:
14025. Incoming energy and water and waste production in-house is
Specific data provided by SunPower for the year 2019. allocated equally among all products through mass allocation. Effects
of primary production of recycled materials allocated to the main
The procedures defined by the PCR regarding the data quality
product in which the material was used. The recycling process and
have been respected according to the following criteria:
transportation of the material is allocated to this analysis.
•Temporal factor: LCI data has been sourced from the database
ecoinvent 3.6, which was updated in 2019, and ELCD, updated in
2018. As such all LCI data has been updated within the last 10
Cut-off criteria:
years All primary data dates from product specific data collections
from within the last 5 years. All major raw materials and all the essential energy is
•Geographical factor: Datasets appropriate to the location of the included. The production process for raw materials and
modelled flow have been selected when available. Certain energy flows that are included with very small amounts (<1%)
datasets have been modified to better reflect the specific energy are not included – this included certain packaging materials
consumptions (see Appendix 2) of certain countries which are not used for the transport of components to the main production
available in the database. When specific data for a country is not facility. The infrastructure relating to the manufacturing facility
available and could not be created, European processes were
has also been exclude as it has negligeable impacts when
selected for flows attributed to Europe, and Global or Rest of
considering the quantity of panels produced.
World flows were used for all other flows.
•Technological factor: Datasets have been selected according to
This cut-off rule does not apply for hazardous materials and
the actual processes used by the manufacturer. For generic
products where no upstream data is available (e.g. packaging), substances.
manufacturing has been modelled according current practices.
NEPD-3087-1726-EN MAXEON 3 MONO-CRYSTALLINE PHOTOVOLTAIC MODULE
3/7
LCA: Scenarios and additional technical information
The following information describe the scenarios in the different modules of the EPD. All data is provided per functional unit
The transports step A4 covers the transport from the factory in Mexico to Europe by boat and truck.
Transport from production place to assembly/user (A4)
Type Capacity utilisation (incl. return) % Type of vehicle Distance km Fuel/Energy Value
consumption (tkm)
Truck 36 EURO5 16-32T 1000 0.0375 kg/tkm 0.09
Boat 50 Transoceanic Freight 8800 0.002 kg/tkm 0.79
Assembly (A5)
The installation of the product requires some metallic fasteners (screws).
The waste from the products packaging is counted in this stage.
Unit Value
Auxiliary (screws) kg 2.34E-05
Material loss kg -
Output materials from waste treatment kg 3.42E-03
Operational energy (B6) and water consumption (B7)
The panels produce electricity during their lifetime but require no inputs/outputs.
To calculate the expected energy production over the lifetime of the panels, the following formula may be used:
25 𝑃
∑ 𝑟𝑎𝑡𝑒𝑑
𝐸𝑛𝑒𝑟𝑔𝑦= 𝑃 × ×(𝜂 ‒0.0025𝑘)
𝑦𝑖𝑒𝑙𝑑 1000 𝑟
𝑘=1
Where:
Energy = Total energy produced by one panel (kWh)
P = Average electricity produced per kWp (kWh/kWp – values available from IEC 61853-3)
yield
P = Energy rating of the panel (kWp)
rated
ƞ = 1 - Efficiency of the panel, assumed to consistently decrease by 0,25% per year for 25 years (initial value at k=1 of 99,75% efficiency
r
assumed for the degradation during the first year)
End of Life (C1, C3, C4)
The end of life scenario taken into account is that of the program
PVCYCLE, to which SunPower subscribe. Panels are sent for
processing and separated into their component parts for recycling
or elimination.
Unit Value
Hazardous waste disposed kg -
Collected as mixed construction waste kg 4,83E-02
Reuse kg -
Recycling kg 4,34E-02
Energy recovery kg 4,88E-03
To landfill kg 1,23E-05
Transport to waste processing (C2)
Fuel/Energy Value
Type Capacity utilisation (incl. return) % Type of vehicle Distance km
Consumption (tkm)
Truck 36 EURO5 16-32T 100 0.0375 kg/tkm 0.084
NEPD-3087-1726-EN MAXEON 3 MONO-CRYSTALLINE PHOTOVOLTAIC MODULE
4/7
LCA: Results
The LCA results show the environmental impacts and resource input and output flows calculated according to EN 15804:2012+A1.
The results are shown per functional unit, which for this declaration is 1Wp, as well as per declared unit, which for this declaration is 1 m².
The LCA results have been calculated using the LCA software SimaPro 9.
System boundaries (X=included, MND=module not declared, MNR=module not relevant)
Beyond the
Assembly
Product stage Use stage End of life stage system
stage
boundaries
5/7
slairetam
waR
tropsnarT
gnirutcafunaM
tropsnarT ylbmessA
esU
ecnanetniaM
riapeR
tnemecalpeR
tnemhsibrufeR
ygrene
lanoitarepO
esu
retaw
lanoitarepO
esu
noitcurtsnoc-eD
noitilomed tropsnarT
gnissecorp
etsaW
lasopsiD
-yrevoceR-esueR laitnetop-gnilcyceR
A1 A2 A3 A4 A5 B1 B2 B3 B4 B5 B6 B7 C1 C2 C3 C4 D
X X X X X MNR MNR MNR MNR MNR MNR MNR MNR X X X X
NEPD-3087-1726-EN MAXEON 3 MONO-CRYSTALLINE PHOTOVOLTAIC MODULE
Environmental impact – Functional Unit
Parameter Unit A1 – A3 A4 A5 C2 C3 C4 D
GWP kg CO2 -eqv 3,42E-01 1,35E-02 8,56E-04 7,97E-04 5,73E-04 6,39E-06 -1,38E-01
ODP kg CFC11-eqv 3,47E-07 2,28E-09 2,07E-11 1,46E-10 5,87E-11 4,56E-14 -9,02E-09
POCP kg C2H4 -eqv 2,89E-04 1,13E-05 1,26E-07 4,15E-07 1,65E-07 2,58E-10 -4,84E-05
AP kg SO2 -eqv 1,86E-03 1,33E-04 7,42E-07 2,55E-06 2,18E-06 2,74E-09 -5,57E-04
EP kg PO43--eqv 2,60E-04 1,37E-05 1,55E-07 4,15E-07 3,05E-07 8,93E-10 -6,88E-05
ADPM kg Sb-eqv 5,23E-05 2,39E-07 3,69E-09 2,18E-08 3,27E-09 3,58E-12 -1,43E-05
ADPE 3,95E+00 1,90E-01 2,06E-03 1,19E-02 5,37E-03 3,83E-06 -1,35E+00 3,83E-06
GWP Global warming potential; ODP Depletion potential of the stratospheric ozone layer; POCP Formation potential of tropospheric
photochemical oxidants; AP Acidification potential of land and water; EP Eutrophication potential; ADPM Abiotic depletion potential for non
fossil resources; ADPE Abiotic depletion potential for fossil resources
Resource use – Functional Unit
Parameter Unit A1 – A3 A4 A5 C2 C3 C4 D
RPEE MJ 1,41E+00 3,53E-03 1,81E-04 1,71E-04 1,73E-03 1,31E-07 -4,73E-01
RPEM MJ 4,11E-02 0,00E+00 0,00E+00 0,00E+00 0,00E+00 0,00E+00 0,00E+00
TPE MJ 1,61E+00 3,53E-03 1,81E-04 1,71E-04 1,73E-03 1,31E-07 -4,73E-01
NRPE MJ 4,56E+00 1,95E-01 2,40E-03 1,21E-02 9,37E-03 4,01E-06 -1,55E+00
NRPM MJ 2,09E-01 0,00E+00 0,00E+00 0,00E+00 0,00E+00 0,00E+00 0,00E+00
TRPE MJ 4,77E+00 1,95E-01 2,39E-03 1,21E-02 9,37E-03 4,01E-06 -1,55E+00
SM kg 2,85E-03 0,00E+00 0,00E+00 0,00E+00 0,00E+00 0,00E+00 0,00E+00
RSF MJ 0,00E+00 0,00E+00 0,00E+00 0,00E+00 0,00E+00 0,00E+00 0,00E+00
NRSF MJ 0,00E+00 0,00E+00 0,00E+00 0,00E+00 0,00E+00 0,00E+00 0,00E+00
W m3 1,63E-02 2,17E-05 2,19E-06 1,25E-06 1,11E-05 1,43E-08 -1,15E-03
RPEE Renewable primary energy resources used as energy carrier; RPEM Renewable primary energy resources used as raw materials;
TPE Total use of renewable primary energy resources; NRPE Non renewable primary energy resources used as energy carrier; NRPM
Non renewable primary energy resources used as materials; TRPE Total use of non renewable primary energy resources; SM Use of
secondary materials; RSF Use of renewable secondary fuels; NRSF Use of non renewable secondary fuels; W Use of net fresh water
End of life - Waste – Functional Unit
Parameter Unit A1 – A3 A4 A5 C2 C3 C4 D
HW kg 2,51E-02 1,46E-04 3,44E-05 7,81E-06 3,28E-05 3,28E-06 -1,34E-03
NHW kg 1,77E-01 7,54E-03 4,35E-04 6,38E-04 1,77E-04 1,56E-07 -3,92E-02
RW kg 1,67E-05 1,31E-06 1,29E-08 8,28E-08 6,79E-08 1,42E-11 -4,46E-06
HW Hazardous waste disposed; NHW Non hazardous waste disposed; RW Radioactive waste disposed
End of life - Output flow – Functional Unit
Parameter Unit A1 – A3 A4 A5 C2 C3 C4 D
CR kg 0,00E+00 0,00E+00 0,00E+00 0,00E+00 0,00E+00 0,00E+00 0,00E+00
MR kg 3,76E-03 0,00E+00 2,21E-03 0,00E+00 4,32E-02 0,00E+00 0,00E+00
MER kg 1,61E-04 0,00E+00 5,68E-04 0,00E+00 4,88E-03 0,00E+00 0,00E+00
EEE MJ 0,00E+00 0,00E+00 0,00E+00 0,00E+00 0,00E+00 0,00E+00 0,00E+00
ETE MJ 5,97E+00 1,99E-01 2,58E-03 1,23E-02 1,11E-02 4,14E-06 -2,02E+00
CR Components for reuse; MR Materials for recycling; MER Materials for energy recovery; EEE Exported electric energy; ETE Exported
thermal energy
Reading example: 9,0 E-03 = 9,0*10-3 = 0,009
NEPD-3087-1726-EN MAXEON 3 MONO-CRYSTALLINE PHOTOVOLTAIC MODULE
6/7
Environmental impact – Declared Unit (1 m²)
Parameter Unit A1 – A3 A4 A5 C2 C3 C4 D
GWP kg CO2 -eqv 7,72E+01 3,04E+00 1,93E-01 1,80E-01 1,29E-01 1,45E-03 -3,12E+01
ODP kg CFC11-eqv 7,84E-05 5,15E-07 4,67E-09 3,30E-08 1,33E-08 1,03E-11 -2,04E-06
POCP kg C2H4 -eqv 6,53E-02 2,56E-03 2,84E-05 9,37E-05 3,73E-05 5,84E-08 -1,09E-02
AP kg SO2 -eqv 5,87E-02 3,09E-03 3,51E-05 9,38E-05 6,90E-05 2,02E-07 -1,55E-02
EP kg PO43--eqv 5,87E-02 3,09E-03 3,51E-05 9,38E-05 6,90E-05 2,02E-07 -1,55E-02
ADPM kg Sb-eqv 1,18E-02 5,39E-05 8,35E-07 4,93E-06 7,38E-07 8,08E-10 -3,23E-03
ADPE 8,92E+02 4,29E+01 4,65E-01 2,69E+00 1,21E+00 8,65E-04 -3,06E+02 8,65E-04
GWP Global warming potential; ODP Depletion potential of the stratospheric ozone layer; POCP Formation potential of tropospheric
photochemical oxidants; AP Acidification potential of land and water; EP Eutrophication potential; ADPM Abiotic depletion potential for non
fossil resources; ADPE Abiotic depletion potential for fossil resources
x
NEPD-3087-1726-EN MAXEON 3 MONO-CRYSTALLINE PHOTOVOLTAIC MODULE
7/7
Resource use – Declared Unit (1 m²)
Parameter Unit A1 – A3 A4 A5 C2 C3 C4 D
RPEE MJ 3,19E+02 7,98E-01 4,09E-02 3,87E-02 3,90E-01 2,95E-05 -1,07E+02
RPEM MJ 9,29E+00 0,00E+00 0,00E+00 0,00E+00 0,00E+00 0,00E+00 0,00E+00
TPE MJ 3,64E+02 7,98E-01 4,09E-02 3,87E-02 3,90E-01 2,95E-05 -1,07E+02
NRPE MJ 1,03E+03 4,41E+01 5,41E-01 2,74E+00 2,12E+00 9,06E-04 -3,50E+02
NRPM MJ 4,73E+01 0,00E+00 0,00E+00 0,00E+00 0,00E+00 0,00E+00 0,00E+00
TRPE MJ 1,08E+03 4,41E+01 5,41E-01 2,74E+00 2,12E+00 9,06E-04 -3,49E+02
SM kg 6,45E-01 0,00E+00 0,00E+00 0,00E+00 0,00E+00 0,00E+00 0,00E+00
RSF MJ 0,00E+00 0,00E+00 0,00E+00 0,00E+00 0,00E+00 0,00E+00 0,00E+00
NRSF MJ 0,00E+00 0,00E+00 0,00E+00 0,00E+00 0,00E+00 0,00E+00 0,00E+00
W m3 3,69E+00 4,91E-03 4,96E-04 2,83E-04 2,50E-03 3,22E-06 -2,61E-01
RPEE Renewable primary energy resources used as energy carrier; RPEM Renewable primary energy resources used as raw materials;
TPE Total use of renewable primary energy resources; NRPE Non renewable primary energy resources used as energy carrier; NRPM
Non renewable primary energy resources used as materials; TRPE Total use of non renewable primary energy resources; SM Use of
secondary materials; RSF Use of renewable secondary fuels; NRSF Use of non renewable secondary fuels; W Use of net fresh water
End of life - Waste – Declared Unit (1 m²)
Parameter Unit A1 – A3 A4 A5 C2 C3 C4 D
HW kg 5,68E+00 3,29E-02 7,78E-03 1,76E-03 7,41E-03 7,42E-04 -3,04E-01
NHW kg 3,99E+01 1,70E+00 9,83E-02 1,44E-01 4,01E-02 3,52E-05 -8,86E+00
RW kg 3,78E-03 2,96E-04 2,91E-06 1,87E-05 1,53E-05 3,21E-09 -1,01E-03
HW Hazardous waste disposed; NHW Non hazardous waste disposed; RW Radioactive waste disposed
End of life - Output flow – Declared Unit (1 m²)
Parameter Unit A1 – A3 A4 A5 C2 C3 C4 D
CR kg 0,00E+00 0,00E+00 0,00E+00 0,00E+00 0,00E+00 0,00E+00 0,00E+00
MR kg 8,49E-01 0,00E+00 5,00E-01 0,00E+00 9,77E+00 0,00E+00 0,00E+00
MER kg 3,63E-02 0,00E+00 1,28E-01 0,00E+00 1,10E+00 0,00E+00 0,00E+00
EEE MJ 0,00E+00 0,00E+00 0,00E+00 0,00E+00 0,00E+00 0,00E+00 0,00E+00
ETE MJ 1,35E+03 4,49E+01 5,82E-01 2,78E+00 2,51E+00 9,35E-04 -4,56E+02
CR Components for reuse; MR Materials for recycling; MER Materials for energy recovery; EEE Exported electric energy; ETE Exported
thermal energy
NEPD-3087-1726-EN MAXEON 3 MONO-CRYSTALLINE PHOTOVOLTAIC MODULE
8/7
Additional Norwegian requirements
Greenhouse gas emission from the use of electricity in the manufacturing phase
National production mix from import, medium voltage (production of transmission lines, in addition to direct emissions and
losses in grid) of applied electricity for the manufacturing process (A3).
Data source Process Amount Unit
Mexico: Ecoinvent v3.6 Electricity, medium voltage {MX}| market for | Cut-off, U 0.583 CO2-eqv/kWh
Electricity, medium voltage {PH}| market for electricity,
Phillipines: Ecoinvent v3.6
medium voltage | Cut-off, U
0.723 CO2-eqv/kWh
Germany: Ecoinvent v3.6 Electricity, medium voltage {DE}| market for | Cut-off, U 0.168 CO2-eqv/kWh
Norway: Ecoinvent v3.6 Electricity, medium voltage {NO}| market for | Cut-off, U 0.020 CO2-eqv/kWh
USA: Ecoinvent v3.6 Electricity, medium voltage {US}| market group for | Cut-off, U 0.558 CO2-eqv/kWh
Dangerous substances
 The product contains no substances given by the REACH Candidate list or the Norwegian priority list.
Indoor environment
No tests have been carried out on the product concerning indoor climate.
Carbon footprint
Carbon footprint has not been worked out for the product.
Bibliography
ISO 14025:2010 Environmental labels and declarations - Type III environmental declarations - Principles and
procedures
ISO 14044:2006 Environmental management - Life cycle assessment - Requirements and guidelines
EN 15804:2012+A1:2013 Sustainability of construction works - Environmental product declaration - Core rules for the
product category of construction products
ISO 21930:2007 Sustainability in building construction - Environmental declaration of building products
SUNPOWER MAXEON 3 MONO-CRYSTALLINE PHOTOVOLTAIC MODULE REPORT
LCA Report
(EVEA, 2021)
Life Cycle Assessment – Modules production in Mexico, Ensenada (Solstyce SAS,
LCA Report
2018)
PCR NPCR 029 version 1.1
PCR – Part B for photovoltaic modules used in the building and construction industry,
including production of cell, wafer, ingot block, solar grade silicon,
solar substrates, solar superstrates and other solar grade semiconductor materials
Other references -
Program operator Phone: +47 23 08 80 00
The Norwegian EPD Foundation
Post Box 5250 Majorstuen, 0303 Oslo e-mail: post@epd-norge.no
Norway web www.epd-norge.no
Publisher Phone: +47 23 08 80 00
The Norwegian EPD Foundation
Post Box 5250 Majorstuen, 0303 Oslo e-mail: post@epd-norge.no
Norway web www.epd-norge.no
Owner of the declaration Phone: +33 7 60 59 84 73
SunPower
Karin.Alberto-
12 Allée du Levant e-mail: Burkhardt@sunpower.co
69890 La Tour de Salvagny m
France web www.sunpower.com
Author of the Life Cycle Assessment Phone: +33 2 28 07 87 00
EVEA
11 rue Voltaire
e-mail: info@evea-conseil.com
44000 Nantes
France web www.evea-conseil.com
NEPD-3087-1726-EN MAXEON 3 MONO-CRYSTALLINE PHOTOVOLTAIC MODULE
9/7
