ver1 2015
ENVIRONMENTAL PRODUCT DECLARATION
in accordance with ISO 14025, ISO 21930 and EN 15804
Owner of the declaration: E.A. Smith AS
Program operator: The Norwegian EPD Foundation
Publisher: The Norwegian EPD Foundation
Declaration number: NEPD-2193-988-EN
Registration number: NEPD-2193-988-EN
ECO Platform reference number: -
Issue date: 14.05.2020
Valid to: 14.05.2025
Steel rebar
E.A. Smith AS (Smith Stål)
Logo
www.epd-norge.no
NEPD-2193-988-EN Steel rebar (korr190122)
General information
Product: Owner of the declaration:
Steel Rebar E.A. Smith AS (Smith Stål)
Contact person: Steve Reinertsen
e-mail: steve.reinertsen@smith.no
Program operator: Manufacturer:
The Norwegian EPD Foundation E.A. Smith AS avd. Smith Stål
Post Box 5250 Majortusten, 0303 Oslo Heggstadmoen 13, 7080 Heimdal
Norway Phone: +47 72 59 25 00
Phone: +47 97722020 e-mail: firmpost@smith.no
e-mail: post@epd-norge.no
Declaration number: Place of production:
NEPD-2193-988-EN Oslo, Holmestrand, Stavanger, Haugesund, Bergen, Ålesund,
Heimdal, Bodø, Harstad and Tromsø (all sites in Norway).
ECO Platform reference number: Management system:
This declaration is based on Product Category Rules: Organisation no:
CEN Standard EN 15804 serves as core PCR
NPCR Part A: Construction products and services 816051142
NPCR 013:2019 Part B for Steel and aluminium construction
Statement of liability: Issue date:
The owner of the declaration shall be liable for the 14.05.2020
underlying information and evidence. EPD Norway shall
not be liable with respect to manufacturerinformation, life
cycle assessment data and evidences.
Valid to:
14.05.2025
Declared unit: Year of study:
per kg steel product 2020
Declared unit with option: Comparability:
EPD of construction products may not be comparable if they not
Per 1 kg steel from cradle to gate comply with EN 15804 and seen in a building context.
Functional unit: The EPD has been worked out by:
Paritosh Chakor Deshpande
Not relevant Annik M Fet
Arron Wilde Tippet
Verification: 10 May 2020
The CEN Norm EN 15804 serves as the core PCR.
Independent verification of the declaration and data,
according to ISO14025:2010
internal external
Approved
Third party verifier:
Michael M. Jenssen, Asplan Viak AS
(Independent verifier approved by EPD Norway)
NEPD-2193-988-EN Steel rebar (korr190122)
2/7
Product
Product description: Technical data:
Steel reinforcement bars (ribbed steel bars) that are made out of hot rolled The product certified is in accordance with standards:
products, transformed into straight ribbed bars, cut and bend, mesh, and NS 3576-1, NS 3576-3 and NS 3576-4
combinations of these (special welded products) by European manufacturers.
Sections are prefabricated by cutting, bending and welding by a Norwegian steel
manufacturer. Reinforcement steel is used in the construction buildings and civil
structures. EPD represents an average value for this product based on several
production sites in Norway. Variance is <10% between sites.
Product specification: Market:
Typical product composition for reinforcement steel is described in the table Norway
below. Typically it consists of more than 99% of steel scrap.
Reference service life, product:
Material kg % Not relevant for cradle to gate
Iron 0,98-0,99 98-99
Carbon 0,005-0,002 0,05-0,02
Manganese 0,03-0,07 0,3-0,7 Reference service life, building:
Silicone 0,02 0,2 Not relevant for cradle to gate
LCA: Calculation rules
Declared unit: System boundary:
Per kg building steel System boundaries are shown in the flowchart. Waste flows, especially cut-
offs from the steel manufacturing in A3, are treated within the module they
occur via system expansion.
Cradle-to-gate LCA was conducted including modules C1-C4 Module D represent a possible system in which the steel output from the
and D as per the requirments presented in 15804:2012 EPD EOL is recycled, from which an environmental credit is attained and given to
guidelines. this system. Module D is calculated as net scrap * LCI for scrap, where the
scrap LCI is calculated as the credit for avoided primary production of steel,
minus the burden of recycling steel scrap to make new steel, multiplied by
the process yield (>1kg scrap is needed to make 1kg new steel). LCI for
scrap has been provided by worldsteel (Worldsteel 2017)
Figure 1: Flowchart showing the system boundaries and processes
system boundary
Data quality: Cut-off criteria:
Data has been collected in accordance with clause 6.3.6 in NPCR Part All major raw materials and all the essential energy is included. The
A for construction products and services. Specific data are used from production process for raw materials and energy flows that are included with
the manufacturer for 2018; when collecting data, efforts have been very small amounts (<1%) are not included. This cut-off rule does not apply
made to create data sets as comprehensive as possible. that no data for hazardous materials and substances.
used >10 years old, or that it is in accordance with 15804. All generic
(background) data has been gathered from PE International Gabi ts
Professional Database and the Ecoinvent database.
Data source: GaBi, Ecoinvent, E.A Smith AS and Supplier EPDs
Allocation:
The allocation is made ​​in accordance with the provisions of EN 15804.
Incoming energy and water and waste production in-house is allocated
equally among all products through mass allocation. Effects of primary
production of recycled materials allocated to the main product in which
the material was used. The recycling process and transportation of the
material is allocated to this analysis. No other products and energy is
produced at Smith Stål facility other than the declared product.
NEPD-2193-988-EN Steel rebar (korr190122)
3/7
LCA: Scenarios and additional technical information
The following information describe the scenarios in the different modules of the EPD.
A4 provides the Transport from the factory gate to the customer. Specific data was obtained from E.A.Smith AS regarding the transport distances and
transport type. Truck Euro 6 are typically used to transport the product within Norway. Transport through truck is also used to dispose other
operational waste and waste lubricant oil from the process, however this fraction accounts for less than 0,01% of total process and hence neglected
through cut-off criteria.
Transport from production place to user (A4)
Type Type of vehicle Distance Fuel/Energy consumption Value (l/t)
Capacity utilisation (incl. return) % km
Truck 85 GLO: Truck EURO 6, 26-28 t 600,02 l/tkm 1,20E+00
Transport in A2 describe the transport of raw material (steel coil rebar and mesh rebar) from various suppliers (from across EU) to E.A. Smith
AS's facility in Norway. Input material from suppliers is transported via ocean-going container ships to Norwegian ports from where Trucks are
used to transport the material to E.A Smith AS plant. The distance travelled and type of transport used was provided by the manufacturer. The
estimates on average % Capacity utilization has also been provided by the manufacturer.
Transport from production place to user (A2)
Type Capacity utilisation (incl. return) % Type of vehicle Distance Fuel/Energy consumption Value (l/t)
Truck 60 GLO: Truck Euro 6 (20-26 Tonnes) 730,0225 l/tkm 1,64E+00
Ship 80 GLO: Container ship, 5000 to 200,000 dwt 14740,0021 l/tkm 3,10E+00
End-of-Life Scenario: 98% recovery rate was assumed considering the high recovery rates of Rebar Steel products (Worldsteel 2017). Among
the total recovered, 98% is assumed for recycling, leaving out 2% fraction to landfilling in Norway.
End of Life (C1, C3, C4)
Transportation scenarios for EOL scenario are based on the approx. Unit Value
distances to the waste management facilities. Other parameters for Hazardous waste disposed kg 0
transporting waste such as capacity utilization, fuel consumption, etc. Collected as mixed construction waste kg 0
are estimated from GaBi ts and ecoinvent v3.4 database Reuse kg 0
Recycling kg 0,98
Energy recovery kg 0
To landfill kg 0,02
Transport to waste processing (C2)
Type Type of vehicle Distanc Fuel/Energy Value
Capacity utilisation (incl. return) %
e km consumption (l/tkm) (l/t)
Truck 65 % GLO: Truck EURO 6, 26-28 t 100 0,0247 2,47E+00
Truck 65 % GLO: Truck EURO 5, 7.5-12 t 100 0,00114 1,14E-01
NEPD-2193-988-EN Steel rebar (korr190122)
4/7
Benefits and loads beyond the system boundaries (D)
Unit Value
Net new scrap kg -0,13
Additional Technical Information
Mer out = 98%
Mer in=110% (Calculated from averaging the value of secondary material from suppliers EPD)
Avoided burden = (Mer out-Mer in)*1,66
Where, 1,66 kg CO2 eq. Is GWP of scrap steel recycle (Worldsteel databse from GaBi ts)
Net credits and burdens for recycling = 0,22 kg CO2 eq.
LCA: Results
The following information describe the scenarios in the different modules of the EPD
System boundaries (X=included, MND= module not declared, MNR=module not relevant)
Beyond the
End of life stage system
boundaries
Environmental impact
Note: Negative value of ADMP (kg Sb eq.) for A1-A3 here is tracked down to the supplier EPD data used for A1. A quick review EPDs suggested that the negative value comes from the
data of Worldsteel due to system expansion and crediting by-products (EAF-dust from recycled material in an electric arc furnace) in the Worldsteel dataset.
Note: There is an inherent flaw in the POCP results in the GaBi 6 software when datasets for trucks have been used with CML 2001. Negative impact results in this category essentially
means that the use of transport will in effect clear smog formation.
GWP Global warming potential; ODP Depletion potential of the stratospheric ozone layer; POCP Formation potential of tropospheric photochemical
oxidants; AP Acidification potential of land and water; EP Eutrophication potential; ADPM Abiotic depletion potential for non fossil resources; ADPE
Abiotic depletion potential for fossil resources
slairetam
waR
tropsnarT
gnirutcafunaM
tropsnarT ylbmessA
The EOL formula from15804 was used to calculate Module D
Product stage Assemby stage Use stage
ecnanetniaM
riapeR
tnemecalpeR tnemhsibrufeR
esu
ygrene
lanoitarepO
A1 A2 A3 A4 A5 B1 B2 B3 B4
esU
esu
retaw
lanoitarepO
noitilomed
noitcurtsnoc-eD tropsnarT
gnissecorp
etsaW
lasopsiD
-gnilcyceR-yrevoceR-esueR
laitnetop
B5 B6 B7 C1 C2 C3 C4 D
X X X X MND MND MND MND MNDMND MND MND X X X X X
Parameter Unit A1-A3 A4 C1 C2 C3 C4 D
GWP kg CO 2 -eqv 3,93E-01 3,55E-03 6,09E-04 7,30E-03 0,00E+00 1,28E-03 2,17E-01
ODP kg CFC11-eqv 6,65E-08 8,85E-19 1,52E-19 1,82E-18 0,00E+00 3,28E-18 -6,59E-16
POCP kg C 2H 4 -eqv 1,11E-04 6,72E-10 2,16E-07 -1,31E-07 0,00E+00 -1,79E-08 1,01E-04
AP kg SO 2 -eqv 1,74E-03 3,17E-06 2,23E-06 6,82E-06 0,00E+00 3,47E-06 4,17E-04
EP kg PO 43--eqv 3,29E-04 7,04E-07 5,39E-07 1,54E-06 0,00E+00 4,85E-07 2,90E-05
ADPM kg Sb-eqv -1,15E-05 3,14E-10 5,39-11 6,44E-10 0,00E+00 2,09E-10 3,64E-06
ADPE MJ 5,30E+00 4,82E-02 8,27E-03 9,89E-02 0,00E+00 1,88E-02 2,03E+00
NEPD-2193-988-EN Steel rebar (korr190122)
5/7
Resource use
Parameter Unit A1-A3 A4 C1 C2 C3 C4 D
RPEE MJ 1,41E+00 2,88E-03 4,94E-04 5,91E-03 0,00E+00 1,28E-03 -1,51E-01
RPEM MJ 7,32E-04 0,00E+00 0,00E+00 0,00E+00 0,00E+00 0,00E+00 3,82E-09
TPE MJ 2,30E+00 2,88E-03 4,94E-04 5,91E-03 0,00E+00 1,28E-03 -1,51E-01
NRPE MJ 4,24E+00 4,85E-02 8,31E-03 9,94E-02 0,00E+00 1,93E-02 1,95E+00
NRPM MJ 1,58E-02 0,00E+00 0,00E+00 0,00E+00 0,00E+00 4,83E-11 -8,84E-11
TRPE MJ 6,14E+00 4,85E-02 8,32E-03 9,94E-02 0,00E+00 1,93E-02 1,95E+00
SM kg 1,11E+00 0,00E+00 0,00E+00 0,00E+00 0,00E+00 0,00E+00 0,00E+00
RSF MJ 6,37E-05 0,00E+00 0,00E+00 0,00E+00 0,00E+00 0,00E+00 0,00E+00
NRSF MJ 2,41E-01 0,00E+00 0,00E+00 0,00E+00 0,00E+00 0,00E+00 0,00E+00
W m3 1,10E-02 4,85E-06 8,32E-07 9,95E-06 0,00E+00 7,35E-07 3,40E-04
RPEE Renewable primary energy resources used as energy carrier; RPEM Renewable primary energy resources used as raw materials; TPE Total
use of renewable primary energy resources; NRPE Non renewable primary energy resources used as energy carrier; NRPM Non renewable primary
energy resources used as materials; TRPE Total use of non renewable primary energy resources; SM Use of secondary materials; RSF Use of
renewable secondary fuels; NRSF Use of non renewable secondary fuels; W Use of net fresh water
End of life - Waste
Parameter Unit A1-A3 A4 C1 C2 C3 C4 D
HW kg 2,20E-02 2,69E-09 4,62E-10 5,52E-09 0,00E+00 3,33E-10 2,50E-07
NHW kg 7,35E-01 4,08E-06 7,01E-07 8,38E-06 0,00E+00 2,00E-02 -2,33E-02
RW kg 1,70E-04 0,00E+00 0,00E+00 0,00E+00 0,00E+00 0,00E+00 0,00E+00
HW Hazardous waste disposed; NHW Non hazardous waste disposed; RW Radioactive waste disposed
End of life - Output flow
Parameter Unit A1-A3 A4 C1 C2 C3 C4 D
CR kg 0 0 0 0 0 0 0
MR kg 1,43E-02 0 0 0 0 9,80E-01 0
MER kg 7,50E-04 0 0 0 0 0 0
EEE MJ 0 0 0 0 0 0 0
ETE MJ 0 0 0 0 0 0 0
*INA: Indicator Not Assessed
CR Components for reuse; MR Materials for recycling; MER Materials for energy recovery; EEE Exported electric energy; ETE Exported thermal
energy
Reading example: 9,0 E-03 = 9,0*10-3 = 0,009
Additional Norwegian requirements
Greenhous gas emission from the use of electricity in the manufacturing phase
The electricity mix used in the manufacturing stage (A3) is the Norwegian electricity grid mix. transformed to low voltage (production of
transmission lines, in addition to direct emissions and losses in grid) for the reference year 2014.
Data source Amount Unit
Econinvent v3.4 (Mar 2020) 0,03 kg CO-eqv/kWh
2
Dangerous substances
The product contains no substances given by the REACH Candidate list or the Norwegian priority list
The product contains substances given by the REACH Candidate list or the Norwegian priority list that are less than 0,1 % by
weight.
The product contain dangerous substances, more then 0,1% by weight, given by the REACH Candidate List or the Norwegian
Priority list, see table.
The product contains no substances given by the REACH Candidate list or the Norwegian priority list. The product is classified as
hazardous waste (Avfallsforskiften, Annex III), see table.
NEPD-2193-988-EN Steel rebar (korr190122)
6/7
Indoor environment
No tests have been carried out on the product concerning indoor climate - Not relevant
Carbon footprint
Carbon footprint has not been worked out for the product.
Bibliography
ISO 14025:2010 Environmental labels and declarations - Type III environmental declarations - Principles and
procedures
ISO 14044:2006 Environmental management - Life cycle assessment - Requirements and guidelines
EN 15804:2012+A1:2013 Sustainability of construction works - Environmental product declaration - Core rules for the product
category of construction products
ISO 21930:2007 Sustainability in building construction - Environmental declaration of building products
NEPD-S-P-00306 EPD 2016. Celsa Nordic Steel
GlobalEPD 001-002 Megasa EPD for Long products of hot rolled structural non-alloy steel coming from electric furnace: ribbed bars. 2018.
EPD-BMG-GB-10.2 and EPD-BS-GB-10.2 Baustahl EPD for reinforcing steel and for reinforcing meshes and lattice girders. 2018.
Deshpande, P.C. (2020) LCA- Report Ribbed bars made from reinforcement steel, in the form of mesh as well as straight and shaped bars
NCPR 2017 Part A NPCR Construction products and services – Part A – April 2017.
NPCR 013 v 3.0 Part B NPCR 013:2019 Part B for steel and aluminium construction products version 3.0.
Worldsteel (2017) World Steel Association Life Cycle Inventory Methodology Report, Brussels: World Steel Association
Program operator Phone: +47 97722020
The Norwegian EPD Foundation
Post Box 5250 Majorstuen, 0303 Oslo e-mail: post@epd-norge.no
Norway web www.epd-norge.no
Publisher Phone: +47 97722020
The Norwegian EPD Foundation
Post Box 5250 Majorstuen, 0303 Oslo e-mail: post@epd-norge.no
Norway web www.epd-norge.no
Owner of the declaration Phone: +47 72 59 24 00
E.A. Smith AS
Company logo
Heggsatdmoen 13 e-mail: firmapost@smith.no
7080 Heimdal web www.smithstal.no
Author of the Life Cycle Assessment Phone: 0047 45 04 09 95
Paritosh Chakor Deshpande Fax
NTNU Gløshaugen e-mail: paritosh.deshpande@ntnu.no
7491 Trondheim web www.ntnu.no
NEPD-2193-988-EN Steel rebar (korr190122)
7/7
