Environmental product declaration
in accordance with ISO 14025 and EN 15804+A2
RLX D FL 80W100-277VACD MB60 AM 3SEABKX
Owner of the declaration: Program operator:
Glamox AS The Norwegian EPD Foundation
Product: Declaration number:
RLX D FL 80W100-277VACD MB60 AM 3SEABKX
NEPD-9331-8926
Declared unit:
1 pcs Registration number:
This declaration is based on Product Category Rules: NEPD-9331-8926
CEN Standard EN 15804:2012+A2:2019 serves as core
Issue date: 07.03.2025
PCR
The Norwegian EPD Foundation IBU PCR - Part B for luminaires, lamps, and components Valid to: 07.03.2030
for luminaires
EPD software:
LCAno EPD generator ID: 823802
1 / 14
General information
Product Owner of the declaration:
RLX D FL 80W100-277VACD MB60 AM 3SEABKX Glamox AS
Contact person: Birger Holo
Phone: +47 97551574
e-mail: birger.holo@glamox.com
Program operator: Manufacturer:
The Norwegian EPD Foundation Glamox AS
Post Box 5250 Majorstuen, 0303 Oslo, Norway Birger Hatlebakks veg 15
Phone: +47 977 22 020 6415 Molde, Norway
web: www.epd-norge.no
Declaration number: Place of production:
Glamox production site Dobczyce (Poland)
NEPD-9331-8926
Jagiellonska 51
32-410 Dobczyce, Poland
This declaration is based on Product Category Rules: Management system:
CEN Standard EN 15804:2012+A2:2019 serves as core PCR ISO 9001, ISO 14001; Molde: ATEX, ISO 80079-34 (IECEx), ISO45001,
IBU PCR - Part B for luminaires, lamps, and components for ISO50001; Kirkenær: ISO 13485; Keila: ISO 45001, ISO 50001;
luminaires Dobczyce: ATEX, ISO 80079-34 (IECEx), Module D 2014/90/EU
Statement of liability: Organisation no:
The owner of the declaration shall be liable for the underlying 912007782
information and evidence. EPD Norway shall not be liable with respect
to manufacturer information, life cycle assessment data and
evidences.​
Declared unit: Issue date:
1 pcs RLX D FL 80W100-277VACD MB60 AM 3SEABKX
07.03.2025
Declared unit with option: Valid to:
A1,A2,A3,A4,A5,B6,C1,C2,C3,C4,D 07.03.2030
Year of study:
2024
Functional unit: Comparability:
1 pc RLX C FL luminaire manufactured in Glamox NT. Transport to EPD of construction products may not be comparable if they not
customer, installed and used according to a specific lighting regime. comply with EN 15804 and seen in a building context.
Including waste treatment in Europe at end-of-life.
General information on verification of EPD from EPD tools: Development and verification of EPD:
Independent verification of data, other environmental information The declaration is created using EPD tool lca.tools ver EPD2021.09,
and the declaration according to ISO 14025:2010, § 8.1.3 and § 8.1.4. developed by LCA.no. The EPD tool is integrated in the company's
Verification of each EPD is made according to EPD-Norway’s management system, and has been approved by EPD Norway.
guidelines for verification and approval requiring that tools are i) NEPDT42
integrated into the company's environmental management system, ii)
the procedures for use of the EPD tool are approved by EPD-Norway, Developer of EPD: Mateusz Tarkowski
and iii) the process is reviewed annually by an independent third
Reviewer of company-specific input data and EPD:​ Grzegorz Kurnik
party verifier. See Appendix G of EPD-Norway's General Programme
Instructions for further information on EPD tools
Verification of EPD tool: Approved:
Independent third party verification of the EPD tool, background data
and test-EPD in accordance with EPDNorway's procedures and
guidelines for verification and approval of EPD tools. Approval
number: NEPDT41.
Third party verifier:
Vito D’Incognito, Take Care International
(no signature required)
2 / 14
Product
Product description:
The RLX D G3 is the third generation RLX D Floodlights. Compared to the RLX D G2, the G3 has in-house developed PSU which enables a
significant increase in power and lumen output from a similar sized product. The enhanced electronic and mechanic capabilities also enables it to
be an excellent platform for Ex Zone1. It’s large connection box, possibility for 2xM20 + 2xM25 cable glands, 0-10V DIM as standard, DALI
options and up to 6mm2 termination blocks, makes it very installation friendly and controllable. The connection box can be filled with gel after
installation, which will fully seal the connection box, and remove it as an inspection point. With up to apx 31.000lm, 240W and beams ranging
from Spot 10 to Wide 110x45, it will solve light challenges in an effective and impressive way, giving customers and end users real added value. -
Flicker Free - Made to handle shocks and vibrations - No maintenance - Designed and produced in Scandinavia - Compact, robust and sealed -
Excellent EMC characteristics - Encapsulated internal electronics - Automatic electronic temperature protection - Dimmable - DALI2 options - No
ballast required - Available for hazardous areas - Corrosion class C5m
Product specification
Materials kg %
Adhesive 0,00030 0,0012
Electronic - Cable 0,56 2,39
Electronic - Connector 0,0038 0,016
Electronic - LED driver 0,21 0,89
Electronic - LED plate 0,47 1,98
Glass - Tempered 0,94 3,98
Plastic - Polyamide 0,0014 0,0060
Plastic - Polymethyl methacrylate
0,21 0,92
(PMMA)
Plastic - Polyoxymethylene (POM) 0,0026 0,011
Plastic - Polypropylene (PP) 0,00030 0,0013
Rubber, synthetic 0,67 2,83
Silicon products 12,11 51,15
Metal - Aluminium alloy 7,45 31,50
Metal - Brass 0,083 0,35
Metal - Steel 0,92 3,90
Metal - Zinc 0,0039 0,016
Plastic - Polyethylene terephthalate
0,000031 0,00013
(PET)
Textile - Polyester 0,00011 0,00047
Total 23,67 100,00
Packaging kg %
Packaging - Cardboard 0,99 92,46
Packaging - Paper 0,08 7,54
Total incl. packaging 24,75 100,00
Technical data:
Please visit the product page on our website for more technical information.
https://www.glamox.com/
Market:
Nordic
Reference service life, product
100 000 hours lifetime for the luminaire according to the technical qualities for the product family.
Reference service life, building or construction works
25 years. Standard service life for installation in Marine, Offshore and Wind.
LCA: Calculation rules
Declared unit:
1 pcs RLX D FL 80W100-277VACD MB60 AM 3SEABKX
Cut-off criteria:
All major raw materials and all the essential energy is included. The production processes for raw materials and energy flows with very small
amounts (less than 1%) can be excluded. These cut-off criteria do not apply for hazardous materials and substances.
Allocation:
The allocation is made in accordance with the provisions of EN 15804. Incoming energy and water and waste production in-house is allocated
equally among all products through mass allocation. Effects of primary production of recycled materials is allocated to the main product in which
the material was used. The recycling process and transportation of the material is allocated to this analysis.
3 / 14
Data quality:
Specific data for the product composition are provided by the manufacturer. The data represent the production of the declared product and were
collected for EPD development in the year of study. Background data is based on EPDs according to EN 15804 and different LCA databases. The
data quality of the raw materials in A1 is presented in the table below.
Materials Source Data quality Year
Adhesive ecoinvent 3.6 Database 2019
Supplier data +
Electronic - Cable Product composition + ecoinvent 3.6 2019
database
Electronic - Connector ecoinvent 3.6 Database 2019
Electronic - LED driver ecoinvent 3.6 Database 2019
Electronic - LED plate ecoinvent 3.6 Database 2019
Glass - Tempered ecoinvent 3.6 Database 2019
Metal - Aluminium alloy Modified ecoinvent 3.6 Database 2019
Metal - Brass ecoinvent 3.6 Database 2019
Metal - Steel ecoinvent 3.6 Database 2019
Metal - Zinc Modified ecoinvent 3.6 Database 2019
Packaging - Cardboard ecoinvent 3.6 Database 2019
Packaging - Paper ecoinvent 3.6 Database 2019
Plastic - Polyamide ecoinvent 3.6 Database 2019
Plastic - Polyethylene terephthalate (PET) ecoinvent 3.6 Database 2019
Plastic - Polymethyl methacrylate (PMMA) ecoinvent 3.6 Database 2019
Plastic - Polyoxymethylene (POM) ecoinvent 3.6 Database 2019
Plastic - Polypropylene (PP) ecoinvent 3.6 Database 2019
Rubber, synthetic ecoinvent 3.6 Database 2019
Silicon products ecoinvent 3.6 Database 2019
Textile - Polyester ecoinvent 3.6 Database 2019
4 / 14
System boundaries (X=included, MND=module not declared, MNR=module not relevant)
Construction Beyond the system
Product stage Use stage End of life stage
installation stage boundaries
A1 A2 A3 A4 A5 B1 B2 B3 B4 B5 B6 B7 C1 C2 C3 C4 D
X X X X X MNR MND MND MND MND X MND X X X X X
System boundary:
The analysis is a cradle-to-grave study of one luminaire manufactured and installed, used according
to a specific lighting regime over a specific lifetime, including waste treatment at end-of-life.
A1-A5 includes the extraction and production of raw materials, transportation to the production site,
the production process itself, transport to the market and assembly.
B6 is the operational energy use stage of the luminaire based on the technical lifetime hours for the
product family and the power consumption of the declared luminaire.
C1-C4 includes de-installation of the luminaire, average transport between
location/application/installation site and waste treatment facility, waste processing and disposal in
Europe. Waste treatment of the product follows the default values provided in EN 50693.
D shows the recyclability of metals and plastics and allows the producers a credit for the net scrap
that is produced at the end of a product’s life. The benefits from recycling of net scrap are described
in formula from EN 15804:2012+A2:2019. Substitution of heat and electricity generated by the
incineration with energy recovery of plastic insulation and other parts is also calculated in module D.
Additional technical information:
Please visit our website www.glamox.com for more technical information.
waR slairetam tropsnarT gnirutcafunaM tropsnarT ylbmessA e​sU ecnanetniaM riapeR tnemecalpeR tnemhsibrufeR lanoitarepO ygrene esu lanoitarepO esu retaw -eD noitcurtsnoc noitilomed tropsnarT etsaW gnissecorp lasopsiD -yrevoceR-esueR laitnetop-gnilcyceR
5 / 14
LCA: Scenarios and additional technical information
The following information describe the scenarios in the different modules of the EPD.
Module A4 = Transport from manufacturing location in Dobczyce to warehouse in Jasin (500 km) + transport to warehouse in Molde (1700 km) +
average distribution into the Nordic market (300 km).
Module B6 = The operational energy use of the luminaire is calculated based on the methodology provided in IBU PCR Part B for luminaires,
lamps, and components for luminaires. The energy consumption model for luminaire used in the PCR follows the application scenarios developed
in EN 15193:2007. To calculate the electricity use of the luminaire, the following scenario parameters have been applied:
- User scenario = Custom *
- Active power of the luminaire (Pa) = 80 watt
- Passive power of the luminaire (Pp) = 0 watt
- Daylight time usage (tD) = 0 hours
- Non-daylight time usage (tN) = 4380 hours
- Standard year time (ty) = 8760 hours
- The occupancy depency factor (FO) = 1 (factor, no unit)
- The daylight dependency factor (FD) = 1 (factor, no unit)
- The product specific constant illuminance factor (FCP) = 1 (factor, no unit)
- The non-daylight dimming factor (FN) = 1 (factor, no unit)
- The application specific empiric lifetime of the luminaire in years (a) = 22,831 years (corresponding to the reference service life of the product).
*The custom user scenario has been developed by Glamox. This scenario is based on our long
industry knowledge of the typical use of this product family and the technical lifetime for the
luminaire.
**The application specific empiric lifetime is 25 years, but since the luminaire has a technical lifetime for 100 000 hours will the estimated 50%
usage yearly exceed this. We therefore use the lifetime hours divided by totally yearly time usage to find our empirical lifetime in this calculation
for energy consumption.
Module C2 = Average transport to Nordic waste treatment facilities (300 km).
Modules C3 and C4:
Waste treatment of the product follows the default values provided in EN 50693, Product Category Rules for life cycle assessments of electronic
and electrical products and systems, table G.4. This table specified how different types of raw materials used in A1 will likely be treated during the
end​of-life of the product. Waste treatments in C3 include material recycling and incineration with and without energy recovery and fly ash
extraction. Disposal in C4 consist of landfilling of different waste
fractions and of ashes.
Module D:
The recyclability of metals, plastics, and electronic components allows the producers a credit for the net scrap that is produced at the end of a
product’s life. The benefits from recycling of net scrap are described in formula from EN 15804:2012+A2:2019. Substitution of heat and electricity
generated by the incineration with energy recovery of plastic insulation and other parts is also calculated in
module D.
The MOW business is of a global nature, that is why it is important to state that the EPD results for these stages are only valid when the products
are being treated in Europe when reaching end of life.
Capacity utilisation Value
Transport from production place to user (A4) Distance (km) Fuel/Energy Consumption Unit
(incl. return) % (Liter/tonne)
Ship, Ferry, Sea (km) 50,0 % 120 0,034 l/tkm 4,08
Truck, 16-32 tonnes, EURO 5 (km) - Europe 36,7 % 2380 0,044 l/tkm 104,72
Assembly (A5) Unit Value
Waste, cardboard and paper, to average treatment
kg 1,071
- A5 including transport (kg)
Operational energy (B6) Unit Value
Electricity, Nordic (kWh) kWh 8000.00
Capacity utilisation Value
Transport to waste processing (C2) Distance (km) Fuel/Energy Consumption Unit
(incl. return) % (Liter/tonne)
Truck, over 32 tonnes, EURO 5 (km) - Europe 53,3 % 300 0,023 l/tkm 6,90
6 / 14
Waste processing (C3) Unit Value
Waste treatment of plastic mixture, incineration
kg 6,63
with energy recovery and fly ash extraction (kg)
Aluminium to recycling (kg) kg 5,22
Brass to recycling (kg) kg 0,050
Waste treatment per kg used electronic
kg 0,57
components, manual seperation (kg)
Copper to recycling (kg) kg 0,19
Waste treatment per kg used PWB, shredding and
separation - C3 (kg) kg 0,68
Waste treatment per kg electronics scrap from
PWB, with components, recycling of metals - C3 kg 0,10
(kg)
Steel to recycling (kg) kg 0,74
Polypropylene (PP) to recycling (kg) kg 0,000061
Waste treatment of polypropylene (PP),
incineration with energy recovery and fly ash kg 0,00012
extraction (kg)
Glass to recycling (kg) kg 0,56
Zinc to recycling (kg) kg 0,0023
Waste treatment per kg electronics scrap from
LED plate, without components, recycling of kg 0,23
copper - C3 (kg)
Disposal (C4) Unit Value
Landfilling of plastic mixture (kg) kg 6,63
Landfilling of ashes from incineration of Plastic
kg 0,23
mixture, process per kg ashes and residues (kg)
Landfilling of aluminium (kg) kg 2,23
Landfilling of brass (kg) kg 0,033
Landfilling of copper (kg) kg 0,12
Landfilling of hazardous waste (kg) kg 0,34
Landfilling of steel (kg) kg 0,18
Landfilling of ashes from incineration of
Polypropylene (PP), process per kg ashes and kg 0,0000036
residues (kg)
Landfilling of glass (kg) kg 0,37
Landfilling of zinc (kg) kg 0,0015
Benefits and loads beyond the system
Unit Value
boundaries (D)
Substitution of electricity, in Norway (MJ) MJ 10,18
Substitution of thermal energy, district heating, in
MJ 154,13
Norway (MJ)
Substitution of primary aluminium with net scrap
kg 4,70
(kg)
Substitution of primary brass with net scrap (kg) kg 0,012
Substitution of primary copper with net scrap (kg) kg 0,19
Substitution of primary metals with net scrap
kg 0,031
from PWB, with components (kg)
Substitution of primary steel with net scrap (kg) kg 0,15
Substitution of polypropylene, PP granulate (kg) kg 0,000061
Substitution of primary glass with net scrap (kg) kg 0,56
Substitution of primary zinc with net scrap (kg) kg 0,0023
Substitution of copper with net scrap from PWB,
kg 0,023
without components (kg)
7 / 14
LCA: Results
The LCA results are presented below for the declared unit defined on page 2 of the EPD document.
Environmental impact
Indicator Unit A1 A2 A3 A4 A5
GWP-total kg CO2 -eq 4,26E+02 3,83E+00 6,47E+01 1,02E+01 1,82E+00
GWP-fossil kg CO2 -eq 4,25E+02 3,83E+00 6,45E+01 1,01E+01 1,73E-02
GWP-biogenic kg CO2 -eq -3,25E-01 1,81E-03 1,71E-01 4,09E-03 1,81E+00
GWP-luluc kg CO2 -eq 9,68E-01 1,40E-03 1,25E-02 3,64E-03 5,73E-06
ODP kg CFC11 -eq 3,99E-05 8,50E-07 2,55E-06 2,30E-06 3,66E-09
AP mol H+ -eq 3,00E+00 1,60E-02 3,88E-01 5,08E-02 8,21E-05
EP-FreshWater kg P -eq 4,04E-02 3,59E-05 7,14E-03 7,84E-05 1,42E-07
EP-Marine kg N -eq 4,46E-01 4,63E-03 4,33E-02 1,46E-02 2,71E-05
EP-Terrestial mol N -eq 5,07E+00 5,13E-02 4,98E-01 1,61E-01 2,94E-04
POCP kg NMVOC -eq 1,46E+00 1,57E-02 1,40E-01 4,80E-02 8,45E-05
ADP-minerals&metals1 kg Sb-eq 5,19E-02 1,37E-04 1,60E-04 2,68E-04 4,22E-07
ADP-fossil1 MJ 4,74E+03 5,72E+01 7,61E+02 1,52E+02 2,42E-01
WDP1 m3 2,38E+04 5,66E+01 3,08E+03 1,42E+02 3,07E-01
Indicator Unit B6 C1 C2 C3 C4 D
GWP-total kg CO2 -eq 1,17E+03 0,00E+00 6,75E-01 1,58E+01 8,70E-01 -4,68E+01
GWP-fossil kg CO2 -eq 1,09E+03 0,00E+00 6,75E-01 1,58E+01 8,69E-01 -4,58E+01
GWP-biogenic kg CO2 -eq 1,99E+01 0,00E+00 2,77E-04 6,46E-04 1,33E-04 -2,07E-01
GWP-luluc kg CO2 -eq 5,95E+01 0,00E+00 1,97E-04 5,70E-04 6,72E-04 -8,28E-01
ODP kg CFC11 -eq 1,18E-04 0,00E+00 1,56E-07 4,27E-08 3,56E-08 -6,51E-02
AP mol H+ -eq 5,01E+00 0,00E+00 2,84E-03 4,02E-03 1,16E-03 -5,03E-01
EP-FreshWater kg P -eq 7,19E-02 0,00E+00 5,15E-06 7,79E-06 4,61E-06 -2,99E-03
EP-Marine kg N -eq 7,91E-01 0,00E+00 8,53E-04 1,75E-03 1,15E-03 -4,89E-02
EP-Terrestial mol N -eq 1,06E+01 0,00E+00 9,43E-03 1,80E-02 4,01E-03 -5,72E-01
POCP kg NMVOC -eq 2,49E+00 0,00E+00 3,03E-03 4,40E-03 1,45E-03 -1,82E-01
ADP-minerals&metals1 kg Sb-eq 1,69E-02 0,00E+00 1,15E-05 2,76E-06 1,22E-06 -3,66E-03
ADP-fossil1 MJ 2,93E+04 0,00E+00 1,05E+01 3,60E+00 3,23E+00 -5,80E+02
WDP1 m3 2,27E+06 0,00E+00 8,05E+00 2,91E+01 3,58E+01 -2,41E+04
GWP-total = Global Warming Potential total; GWP-fossil = Global Warming Potential fossil fuels; GWP-biogenic = Global Warming Potential biogenic; GWP-luluc =
Global Warming Potential land use and land use change; ODP = Depletion potential of the stratospheric ozone layer; AP = Acidification potential, Accumulated
Exceedance; EP-freshwater = Eutrophication potential, fraction of nutrients reaching freshwater end compartment: EP-marine = Eutrophication potential, fraction of
nutrients reaching marine end compartment; EP-terrestrial = Eutrophication potential, Accumulated Exceedance; POCP = Formation potential of tropospheric ozone;
ADP-minerals&metals = Abiotic depletion potential for non-fossil resources; ADP-fossil = Abiotic depletion for fossil resources potential; WDP = Water (user)
deprivation potential, deprivation-weighted water consumption
"Reading example: 9,0 E-03 = 9,0*10-3 = 0,009"
*INA Indicator Not Assessed
1. The results of this environmental impact indicator shall be used with care as the uncertainties on these results are high or as there is limited experienced with the
indicator
Remarks to environmental impacts
8 / 14
A luminaire is a product that consumes energy during the use phase. Combined with a relatively long expected lifetime and the environmental
impact of generating electricity, the use phase (B6) will normally be the most contributing stage to the overall environmental impact of the
declared unit. It is important to be aware that the actual calculations of the effect of B6 is particularly sensitive to which use scenario and fuel
source that is chosen.
9 / 14
Additional environmental impact indicators
Indicator Unit A1 A2 A3 A4 A5
PM Disease incidence 2,74E-05 2,59E-07 6,35E-07 7,16E-07 1,21E-09
IRP2 kgBq U235 -eq 1,16E+01 2,47E-01 6,37E-01 6,65E-01 1,04E-03
ETP-fw1 CTUe 2,01E+04 4,73E+01 7,60E+02 1,11E+02 3,23E-01
HTP-c1 CTUh 4,97E-07 7,06E-10 2,40E-08 0,00E+00 1,00E-11
HTP-nc1 CTUh 1,50E-05 4,96E-08 9,54E-07 1,21E-07 4,06E-10
SQP1 dimensionless 1,24E+03 3,72E+01 1,98E+02 1,03E+02 1,63E-01
Indicator Unit B6 C1 C2 C3 C4 D
PM Disease incidence 2,66E-05 0,00E+00 5,94E-08 1,91E-08 2,19E-08 -3,85E-06
IRP2 kgBq U235 -eq 6,69E+02 0,00E+00 4,59E-02 1,30E-02 1,45E-02 -2,50E+00
ETP-fw1 CTUe 3,67E+04 0,00E+00 7,68E+00 3,57E+01 1,60E+03 -2,39E+03
HTP-c1 CTUh 8,56E-07 0,00E+00 0,00E+00 3,00E-09 4,38E-10 -1,24E-07
HTP-nc1 CTUh 2,25E-05 0,00E+00 7,43E-09 1,65E-07 4,76E-09 -2,60E-06
SQP1 dimensionless 2,21E+04 0,00E+00 1,20E+01 7,00E-01 9,49E+00 -1,21E+02
PM = Particulate Matter emissions; IRP = Ionizing radiation – human health; ETP-fw = Eco toxicity – freshwater; HTP-c = Human toxicity – cancer effects; HTP-nc =
Human toxicity – non cancer effects; SQP = Potential Soil Quality Index (dimensionless)
"Reading example: 9,0 E-03 = 9,0*10-3 = 0,009"
*INA Indicator Not Assessed
1. The results of this environmental impact indicator shall be used with care as the uncertainties on these results are high or as there is limited experienced with the
indicator
2. This impact category deals mainly with the eventual impact of low dose ionizing radiation on human health of the nuclear fuel cycle. It does not consider effects due
to possible nuclear accidents, occupational exposure nor due to radioactive waste disposal in underground facilities. Potential ionizing radiation from the soil, from
radon and from some construction materials is also not measured by this indicator.
10 / 14
Resource use
Indicator Unit A1 A2 A3 A4 A5
PERE MJ 5,02E+02 9,11E-01 5,91E+01 2,12E+00 3,99E-03
PERM MJ 2,82E+01 0,00E+00 0,00E+00 0,00E+00 -3,01E+01
PERT MJ 5,31E+02 9,11E-01 5,91E+01 2,12E+00 -3,01E+01
PENRE MJ 4,59E+03 5,72E+01 7,61E+02 1,52E+02 2,43E-01
PENRM MJ 1,49E+02 0,00E+00 0,00E+00 0,00E+00 0,00E+00
PENRT MJ 4,74E+03 5,72E+01 7,61E+02 1,52E+02 2,43E-01
SM kg 1,80E+00 0,00E+00 0,00E+00 0,00E+00 0,00E+00
RSF MJ 2,81E+00 3,03E-02 3,03E+00 7,54E-02 1,32E-04
NRSF MJ 1,46E+00 5,67E-02 4,75E+00 2,67E-01 5,46E-04
FW m3 4,32E+00 6,96E-03 1,53E+00 1,58E-02 1,14E-04
Indicator Unit B6 C1 C2 C3 C4 D
PERE MJ 2,89E+04 0,00E+00 1,32E-01 3,82E-01 4,72E-01 -2,76E+02
PERM MJ 0,00E+00 0,00E+00 0,00E+00 0,00E+00 0,00E+00 0,00E+00
PERT MJ 2,89E+04 0,00E+00 1,32E-01 3,82E-01 4,72E-01 -2,76E+02
PENRE MJ 2,98E+04 0,00E+00 1,05E+01 3,60E+00 3,24E+00 -5,80E+02
PENRM MJ 0,00E+00 0,00E+00 0,00E+00 -1,50E+02 0,00E+00 -2,03E-03
PENRT MJ 2,98E+04 0,00E+00 1,05E+01 -1,46E+02 3,24E+00 -5,80E+02
SM kg 0,00E+00 0,00E+00 0,00E+00 0,00E+00 7,36E-03 1,29E-01
RSF MJ 2,92E+02 0,00E+00 4,62E-03 6,02E-03 4,56E-03 -7,52E-02
NRSF MJ 0,00E+00 0,00E+00 1,55E-02 -1,35E-04 6,69E-02 -4,19E+00
FW m3 1,31E+02 0,00E+00 1,20E-03 1,96E-02 3,52E-03 -1,18E+00
PERE = Use of renewable primary energy excluding renewable primary energy resources used as raw materials; PERM = Use of renewable primary energy resources used
as raw materials; PERT = Total use of renewable primary energy resources; PENRE = Use of non renewable primary energy excluding non-renewable primary energy
resources used as raw materials; PENRM = Use of non renewable primary energy resources used as raw materials; PENRT = Total use of non renewable primary energy
resources; SM = Use of secondary materials; RSF = Use of renewable secondary fuels; NRSF = Use of non-renewable secondary fuels; FW = Net use of fresh water
"Reading example: 9,0 E-03 = 9,0*10-3 = 0,009"
*INA Indicator Not Assessed
11 / 14
End of life - Waste
Indicator Unit A1 A2 A3 A4 A5
HWD kg 2,46E+00 4,51E-03 1,78E-01 7,72E-03 0,00E+00
NHWD kg 6,28E+01 2,57E+00 3,88E+00 7,09E+00 1,07E+00
RWD kg 1,02E-02 3,83E-04 5,97E-04 1,04E-03 0,00E+00
Indicator Unit B6 C1 C2 C3 C4 D
HWD kg 2,75E+00 0,00E+00 5,75E-04 6,12E-05 4,44E-01 1,59E-01
NHWD kg 1,82E+02 0,00E+00 9,13E-01 8,37E-02 9,64E+00 -1,31E+01
RWD kg 3,08E-01 0,00E+00 7,17E-05 3,22E-06 1,61E-05 -2,34E-03
HWD = Hazardous waste disposed; NHWD = Non-hazardous waste disposed; RWD = Radioactive waste disposed
"Reading example: 9,0 E-03 = 9,0*10-3 = 0,009"
*INA Indicator Not Assessed
End of life - Output flow
Indicator Unit A1 A2 A3 A4 A5
CRU kg 0,00E+00 0,00E+00 0,00E+00 0,00E+00 0,00E+00
MFR kg 0,00E+00 0,00E+00 2,06E+00 0,00E+00 9,97E-01
MER kg 0,00E+00 0,00E+00 8,62E-01 0,00E+00 7,49E-02
EEE MJ 0,00E+00 0,00E+00 6,92E-01 0,00E+00 6,13E-02
EET MJ 0,00E+00 0,00E+00 1,05E+01 0,00E+00 9,27E-01
Indicator Unit B6 C1 C2 C3 C4 D
CRU kg 0,00E+00 0,00E+00 0,00E+00 0,00E+00 0,00E+00 0,00E+00
MFR kg 0,00E+00 0,00E+00 0,00E+00 6,77E+00 5,95E-04 -5,77E-03
MER kg 0,00E+00 0,00E+00 0,00E+00 6,63E+00 1,45E-05 -7,54E-04
EEE MJ 0,00E+00 0,00E+00 0,00E+00 1,02E+01 9,44E-04 -2,10E-03
EET MJ 0,00E+00 0,00E+00 0,00E+00 1,54E+02 1,43E-02 -3,18E-02
CRU = Components for re-use; MFR = Materials for recycling; MER = Materials for energy recovery; EEE = Exported energy electrical; EET = Exported energy thermal
"Reading example: 9,0 E-03 = 9,0*10-3 = 0,009"
*INA Indicator Not Assessed
Biogenic Carbon Content
Indicator Unit At the factory gate
Biogenic carbon content in product kg C 0,00E+00
Biogenic carbon content in accompanying packaging kg C 4,93E-01
Note: 1 kg biogenic carbon is equivalent to 44/12 kg CO2
12 / 14
Additional requirements
Greenhouse gas emissions from the use of electricity in the manufacturing phase
National production mix from import, low voltage (production of transmission lines, in addition to direct emissions and losses in grid) of applied
electricity for the manufacturing process (A3).
Electricity mix Source Amount Unit
Electricity, Poland (kWh) ecoinvent 3.6 1060,47 g CO2-eq/kWh
Dangerous substances
The product contains no substances given by the REACH Candidate list.
Indoor environment
Additional Environmental Information
Additional environmental impact indicators required in NPCR Part A for construction products
Indicator Unit A1 A2 A3 A4 A5
GWPIOBC kg CO2 -eq 4,28E+02 3,83E+00 6,64E+01 1,02E+01 1,73E-02
Indicator Unit B6 C1 C2 C3 C4 D
GWPIOBC kg CO2 -eq 1,58E+03 0,00E+00 6,75E-01 1,58E+01 8,96E-01 -4,47E+01
GWP-IOBC: Global warming potential calculated according to the principle of instantaneous oxidation. In order to increase the transparency of biogenic carbon​
contribution to climate impact, the indicator GWP-IOBC is required as it declares climate impacts calculated according to the principle of instantaneous oxidation.​
GWP-IOBC is also referred to as GWP-GHG in context to Swedish public procurement legislation.
13 / 14
Bibliography
ISO 14025:2010. Environmental labels and declarations - Type III environmental declarations - Principles and procedures. International
Organization for Standardization.
ISO 14044:2006. Environmental management - Life cycle assessment - Requirements and guidelines. International Organization for
Standardization.
EN 15804:2012+A2:2019. Environmental product declaration - Core rules for the product category of construction products. European
Committee for Standardization.
ISO 21930:2017. Sustainability in buildings and civil engineering works - Core rules for environmental product declarations of construction
products. International Organization for Standardization.
EN 50693:2019. Product category rules for life cycle assessments of electronic and electrical products and systems. European Committee for
Standardization.
Ecoinvent v3, 2019. Allocation, cut-off by classification. Swiss Centre of Life Cycle Inventories.
Iversen et al., (2021). eEPD v2021.09, background information for EPD generator tool system verification, LCA.no. Report number: 07.21. System
verification report.
Philis et al., (2022). EPD generator for IBU PCR part B for luminaires, lamps, and components for luminaires, background information for EPD
generator application and LCA data, LCA.no. Report number: 04.22. PCR verification report.
EPD Norway (2022). NPCR Part A: Construction products and services. The Norwegian EPD foundation. Version 2.0 published 24.03.2021.
IBU (2017). PCR part B for luminaires, lampes and components for luminaires. Institut Bauen und Umwelt e.V. Version 1.7, published 30.11.2017.
Life cycle inventory (LCI) report for RRLX D FL 80W100-277VACD MB60 AM 3SEABKX, Glamox, February 2024.
Program operator and publisher Phone: +47 977 22 020
The Norwegian EPD Foundation e-mail: post@epd-norge.no
Post Box 5250 Majorstuen, 0303 Oslo, Norway web: www.epd-norge.no
Owner of the declaration: Phone: +47 97551574
Glamox AS e-mail: birger.holo@glamox.com
Birger Hatlebakks veg 15, 6415 Molde, Norway web: https://www.glamox.com
Author of the Life Cycle Assessment Phone: +47 916 50 916
LCA.no AS e-mail: post@lca.no
Dokka 6A, 1671 Kråkerøy, Norway web: www.lca.no
Developer of EPD generator Phone: +47 916 50 916
LCA.no AS e-mail: post@lca.no
Dokka 6A, 1671 Kråkerøy, Norway web: www.lca.no
ECO Platform web: www.eco-platform.org
ECO Portal web: ECO Portal
14 / 14
