Environmental product declaration
in accordance with ISO 14025 and EN 15804+A2
U12-32 - Korg Park bench
Owner of the declaration: Program operator:
Nola Industrier Aktiebolag The Norwegian EPD Foundation
Product: Declaration number:
U12-32 - Korg Park bench
Registration number:
Declared unit:
1 pcs Issue date:
This declaration is based on Product Category Rules: Valid to:
CEN Standard EN 15804:2012+A2:2019 serves as core
EPD software:
PCR
LCAno EPD generator ID: 618212
The Norwegian EPD Foundation NPCR 026:2022 Part B for Furniture
1 / 12
General information
Product Owner of the declaration:
U12-32 - Korg Park bench Nola Industrier Aktiebolag
Contact person: Anders Åkesson
Phone: 08-702 19 60
e-mail: anders.akesson@nola.se
Program operator: Manufacturer:
The Norwegian EPD Foundation Nola Industrier Aktiebolag
Post Box 5250 Majorstuen, 0303 Oslo, Norway
Phone: +47 977 22 020
web: www.epd-norge.no
Declaration number: Place of production:
Nola Industrier Aktiebolag
Blekingegatan 26
118 56 Stockholm, Sweden
This declaration is based on Product Category Rules: Management system:
CEN Standard EN 15804:2012+A2:2019 serves as core PCR
NPCR 026:2022 Part B for Furniture
Statement of liability: Organisation no:
The owner of the declaration shall be liable for the underlying 556207-4442
information and evidence. EPD Norway shall not be liable with respect
to manufacturer information, life cycle assessment data and
evidences.​
Declared unit: Issue date:
1 pcs U12-32 - Korg Park bench
Declared unit (cradle to gate) with option: Valid to:
A1-A3,A4,A5,B2,B3,B4,C1,C2,C3,C4,D
Year of study:
2022
Functional unit: Comparability:
1 Korg Park bench, from the Korg furniture series, as delivered to the EPD of construction products may not be comparable if they not
final customer. comply with EN 15804 and seen in a building context.
General information on verification of EPD from EPD tools: Development and verification of EPD:
Independent verification of data, other environmental information The declaration is created using EPD tool lca.tools ver EPD2022.03,
and the declaration according to ISO 14025:2010, § 8.1.3 and § 8.1.4. developed by LCA.no. The EPD tool is integrated in the company's
Verification of each EPD is made according to EPD-Norway’s management system, and has been approved by EPD Norway.
guidelines for verification and approval requiring that tools are i)
integrated into the company's environmental management system, ii) Developer of EPD: Joachim Henriksson
the procedures for use of the EPD tool are approved by EPD-Norway,
Reviewer of company-specific input data and EPD: Anders Åkesson
and iii) the process is reviewed annually by an independent third
party verifier. See Appendix G of EPD-Norway's General Programme
Instructions for further information on EPD tools
Verification of EPD tool: Approved:
Independent third party verification of the EPD tool, background data
and test-EPD in accordance with EPDNorway's procedures and
guidelines for verification and approval of EPD tools.
Håkon Hauan, CEO EPD-Norge
Third party verifier:
Elisabet Amat, GREENIZE projects
(no signature required)
2 / 12
Product
Product description:
Korg park bench is part of the Korg furniture group. Korg is a neat, expressive wire furniture for outdoor use, anchored in a cylindrical base. The
thread's thin, vertical lines and checkered seat interact with each other and create a clear graphic expression. At the same time, the function of the
material makes it easy for water to drain off. The sofa can also be assembled into several parts and variations, see Korg building system.
Product specification
U12-32 - Korg Park bench
Width: 130 cm
Height: 88 cm
Sitting height: 45 cm
Depth: 61 cm
Recycled
Recycled share in share in
Materials kg %
material (kg) material
(%)
Powder coating 0,25 0,98 0,00 0,00
Zinc 0,33 1,29 0,00 0,00
Metal - Steel 24,85 96,99 0,00 0,00
Metal - Stainless steel 0,19 0,74 0,04 21,83
Total 25,62 100,00 0,04
Recycled
Recycled share in share in
Packaging kg %
material (kg) material
(%)
Packaging -
2,50 12,78 0,00 0,00
Cardboard
Packaging - Pallet 16,88 86,25 0,00 0,00
Packaging - Plastic 0,19 0,97 0,00 0,00
Total incl. packaging 45,19 100,00 0,04
Technical data:
Market:
Global.
Reference service life, product
15 years.
Reference service life, building
LCA: Calculation rules
Declared unit:
1 pcs U12-32 - Korg Park bench
Cut-off criteria:
All major raw materials and all the essential energy is included. The production processes for raw materials and energy flows with very small
amounts (less than 1%) are not included. These cut-off criteria do not apply for hazardous materials and substances.
Energy flows and materials representing less than 1% of the total are excluded. Cut-off does not apply for REACH materials.
Allocation:
The allocation is made in accordance with the provisions of EN 15804. Incoming energy and water and waste production in-house is allocated
equally among all products through mass allocation. Effects of primary production of recycled materials is allocated to the main product in which
the material was used. The recycling process and transportation of the material is allocated to this analysis. Allocation as per EN 15804.
Impacts from primary production of virgin material are assigned to respective component production and includes transportation.
Impacts from repair and replacement are not included in the use stage, as the materials used in the product are designed to last longer than the
stated lifespan
Impacts from primary production of recycled materials are assigned to respective component production, and includes recycling and
transportation processes.
Emissions from disposal of the product are included and allocated per material. Energy recovery from incineration of relevant materials is included
and allocated on a national level.
3 / 12
Data quality:
Specific data for the product composition are provided by the manufacturer. They represent the production of the declared product and were
collected for EPD development in the year of study. Background data is based on registered EPDs according to EN 15804, Ostfold Research
databases, ecoinvent and other LCA databases. The data quality of the raw materials in A1 is presented in the table below.​
Data has been gathered from sub suppliers and public, current, published EPDs or ecoinvent 3.6 database.
Materials Source Data quality Year
Metal - Stainless steel ecoinvent 3.6 Database 2019
Metal - Steel ecoinvent 3.6 Database 2019
Packaging - Cardboard Modified ecoinvent 3.6 Database 2019
Packaging - Pallet ecoinvent 3.6 Database 2019
Packaging - Plastic ecoinvent 3.6 Database 2019
Powder coating Ecoinvent 3.6 Database 2019
Zinc ecoinvent 3.6 Database 2019
4 / 12
System boundaries (X=included, MND=module not declared, MNR=module not relevant)
Construction Beyond the system
Product stage Use stage End of life stage
installation stage boundaries
A1 A2 A3 A4 A5 B1 B2 B3 B4 B5 B6 B7 C1 C2 C3 C4 D
X X X X X MND X X X MND MND MND X X X X X
System boundary:
Sweden
Additional technical information:
https://nola.se/produkter/korg-tradsoffa/
waR slairetam tropsnarT gnirutcafunaM tropsnarT ylbmessA e​sU ecnanetniaM riapeR tnemecalpeR tnemhsibrufeR lanoitarepO ygrene esu lanoitarepO esu retaw -eD noitcurtsnoc noitilomed tropsnarT etsaW gnissecorp lasopsiD -yrevoceR-esueR laitnetop-gnilcyceR
5 / 12
LCA: Scenarios and additional technical information
The following information describe the scenarios in the different modules of the EPD.
Production scenario assumes production in Sweden at sub-suppliers with transport of materials and components between certain production
steps.
Usage scenario assumes no repair or replacement and minimal maintenance during the 15 year lifespan of the product, as materials and surface
treatments are selected to require servicing during lifetime of product. The installation location is assumed to be within Sweden.
Capacity utilisation Value
Transport from production place to user (A4) Distance (km) Fuel/Energy Consumption Unit
(incl. return) % (Liter/tonne)
Truck, over 32 tonnes, EURO 5 (km) 53,3 % 400 0,023 l/tkm 9,20
Assembly (A5) Unit Value
Waste, packaging, corrugated board box, 0 %
kg 2,50
recycled, to average treatment (kg)
Waste, packaging, Pallet, EUR wooden pallet,
kg 16,88
single use, average treatment (kg)
Waste, packaging, plastic film (LDPE), to average
kg 0,19
treatment - A5 (kg)
Capacity utilisation Value
Transport to waste processing (C2) Distance (km) Fuel/Energy Consumption Unit
(incl. return) % (Liter/tonne)
Truck, 16-32 tonnes, EURO 5 (km) 36,7 % 50 0,044 l/tkm 2,20
Waste processing (C3) Unit Value
Waste, materials to recycling (kg) kg 8,50
Waste treatment per kg Scrap steel, incineration
kg 25,04
with fly ash extraction (kg)
Waste treatment per kg Non-hazardous waste,
kg 0,58
incineration with fly ash extraction - C3 (kg)
Disposal (C4) Unit Value
Landfilling of ashes and residues from
kg 16,54
incineration of Scrap steel (kg)
Landfilling of ashes from incineration of Non-
hazardous waste, process per kg ashes and kg 0,14
residues - C4 (kg)
Benefits and loads beyond the system
Unit Value
boundaries (D)
Substitution of primary steel with net scrap (kg) kg 8,48
Substitution of electricity (MJ) MJ 0,34
Substitution of thermal energy, district heating
MJ 5,21
(MJ)
6 / 12
LCA: Results
The LCA results are presented below for the declared unit defined on page 2 of the EPD document.
Environmental impact
Indicator Unit A1-A3 A4 A5 B2 B3
GWP-total kg CO2 -eq 5,80E+01 1,64E+00 3,03E+01 0 0
GWP-fossil kg CO2 -eq 8,71E+01 1,64E+00 5,10E-01 0 0
GWP-biogenic kg CO2 -eq -2,95E+01 6,74E-04 2,98E+01 0 0
GWP-luluc kg CO2 -eq 4,26E-01 4,80E-04 1,31E-04 0 0
ODP kg CFC11 -eq 7,46E-06 3,80E-07 8,20E-08 0 0
AP mol H+ -eq 4,72E-01 6,90E-03 3,86E-03 0 0
EP-FreshWater kg P -eq 5,27E-03 1,25E-05 5,81E-06 0 0
EP-Marine kg N -eq 9,38E-02 2,08E-03 1,65E-03 0 0
EP-Terrestial mol N -eq 1,08E+00 2,30E-02 1,75E-02 0 0
POCP kg NMVOC -eq 4,32E-01 7,38E-03 4,53E-03 0 0
ADP-minerals&metals1 kg Sb-eq 2,72E-02 2,81E-05 8,43E-06 0 0
ADP-fossil1 MJ 1,54E+03 2,55E+01 5,96E+00 0 0
WDP1 m3 6,65E+04 1,96E+01 9,15E+00 0 0
Indicator Unit B4 C1 C2 C3 C4 D
GWP-total kg CO2 -eq 0 0 3,77E-01 1,48E+00 1,78E-01 -9,37E+00
GWP-fossil kg CO2 -eq 0 0 3,77E-01 1,48E+00 1,78E-01 -9,36E+00
GWP-biogenic kg CO2 -eq 0 0 1,54E-04 2,47E-03 1,35E-04 -5,21E-03
GWP-luluc kg CO2 -eq 0 0 1,32E-04 5,68E-05 5,49E-05 -5,22E-03
ODP kg CFC11 -eq 0 0 8,59E-08 2,02E-08 5,68E-08 -2,20E-03
AP mol H+ -eq 0 0 1,54E-03 1,05E-03 1,29E-03 -4,66E-02
EP-FreshWater kg P -eq 0 0 2,96E-06 4,83E-06 1,74E-06 -5,77E-04
EP-Marine kg N -eq 0 0 4,57E-04 3,94E-04 4,61E-04 -9,68E-03
EP-Terrestial mol N -eq 0 0 5,05E-03 4,22E-03 5,10E-03 -9,90E-02
POCP kg NMVOC -eq 0 0 1,55E-03 1,25E-03 1,47E-03 -4,70E-02
ADP-minerals&metals1 kg Sb-eq 0 0 1,02E-05 1,15E-06 3,18E-06 -1,61E-04
ADP-fossil1 MJ 0 0 5,68E+00 1,43E+00 4,19E+00 -7,90E+01
WDP1 m3 0 0 5,42E+00 2,73E-01 7,59E+00 4,79E+02
GWP-total = Global Warming Potential total; GWP-fossil = Global Warming Potential fossil fuels; GWP-biogenic = Global Warming Potential biogenic; GWP-luluc =
Global Warming Potential land use and land use change; ODP = Depletion potential of the stratospheric ozone layer; AP = Acidification potential, Accumulated
Exceedance; EP-freshwater = Eutrophication potential, fraction of nutrients reaching freshwater end compartment: EP-marine = Eutrophication potential, fraction of
nutrients reaching marine end compartment; EP-terrestrial = Eutrophication potential, Accumulated Exceedance; POCP = Formation potential of tropospheric ozone;
ADP-minerals&metals = Abiotic depletion potential for non-fossil resources; ADP-fossil = Abiotic depletion for fossil resources potential; WDP = Water (user)
deprivation potential, deprivation-weighted water consumption
"Reading example: 9,0 E-03 = 9,0*10-3 = 0,009"
*INA Indicator Not Assessed
1. The results of this environmental impact indicator shall be used with care as the uncertainties on these results are high or as there is limited experienced with the
indicator
Remarks to environmental impacts
7 / 12
Additional environmental impact indicators
Indicator Unit A1-A3 A4 A5 B2 B3
PM Disease incidence 7,82E-06 1,45E-07 4,78E-08 0 0
IRP2 kgBq U235 -eq 2,40E+01 1,12E-01 2,20E-02 0 0
ETP-fw1 CTUe 4,40E+03 1,87E+01 6,89E+00 0 0
HTP-c1 CTUh 6,33E-07 0,00E+00 7,00E-10 0 0
HTP-nc1 CTUh 3,09E-06 1,81E-08 3,34E-08 0 0
SQP1 dimensionless 3,68E+03 2,93E+01 3,48E+00 0 0
Indicator Unit B4 C1 C2 C3 C4 D
PM Disease incidence 0 0 2,71E-08 4,43E-08 2,38E-08 -7,90E-07
IRP2 kgBq U235 -eq 0 0 2,48E-02 4,41E-03 1,67E-02 3,08E-02
ETP-fw1 CTUe 0 0 4,18E+00 1,32E+01 2,38E+00 -5,23E+02
HTP-c1 CTUh 0 0 0,00E+00 1,29E-09 8,30E-11 -4,49E-08
HTP-nc1 CTUh 0 0 4,52E-09 8,17E-09 2,14E-09 9,74E-07
SQP1 dimensionless 0 0 3,92E+00 3,47E-01 9,05E+00 -8,77E+00
PM = Particulate Matter emissions; IRP = Ionizing radiation – human health; ETP-fw = Eco toxicity – freshwater; HTP-c = Human toxicity – cancer effects; HTP-nc =
Human toxicity – non cancer effects; SQP = Soil Quality (dimensionless)
"Reading example: 9,0 E-03 = 9,0*10-3 = 0,009"
*INA Indicator Not Assessed
1. The results of this environmental impact indicator shall be used with care as the uncertainties on these results are high or as there is limited experienced with the
indicator
2. This impact category deals mainly with the eventual impact of low dose ionizing radiation on human health of the nuclear fuel cycle. It does not consider effects due
to possible nuclear accidents, occupational exposure nor due to radioactive waste disposal in underground facilities. Potential ionizing radiation from the soil, from
radon and from some construction materials is also not measured by this indicator.
8 / 12
Resource use
Indicator Unit A1-A3 A4 A5 B2 B3
PERE MJ 6,03E+02 3,22E-01 1,21E-01 0 0
PERM MJ 2,74E+02 0,00E+00 -2,74E+02 0 0
PERT MJ 8,77E+02 3,22E-01 -2,74E+02 0 0
PENRE MJ 1,53E+03 2,56E+01 5,96E+00 0 0
PENRM MJ 8,07E+00 0,00E+00 -8,07E+00 0 0
PENRT MJ 1,54E+03 2,56E+01 -2,10E+00 0 0
SM kg 4,15E-02 0,00E+00 0,00E+00 0 0
RSF MJ 2,46E+00 1,12E-02 3,55E-03 0 0
NRSF MJ 6,07E+01 3,77E-02 3,78E-02 0 0
FW m3 1,43E+00 2,91E-03 4,18E-03 0 0
Indicator Unit B4 C1 C2 C3 C4 D
PERE MJ 0 0 8,01E-02 8,25E-02 7,46E-02 -9,04E+00
PERM MJ 0 0 0,00E+00 0,00E+00 0,00E+00 0,00E+00
PERT MJ 0 0 8,01E-02 8,25E-02 7,46E-02 -9,04E+00
PENRE MJ 0 0 5,68E+00 1,49E+00 4,19E+00 -7,90E+01
PENRM MJ 0 0 0,00E+00 0,00E+00 0,00E+00 0,00E+00
PENRT MJ 0 0 5,68E+00 1,49E+00 4,19E+00 -7,90E+01
SM kg 0 0 0,00E+00 0,00E+00 0,00E+00 0,00E+00
RSF MJ 0 0 2,87E-03 1,72E-03 1,98E-03 3,37E-01
NRSF MJ 0 0 1,02E-02 0,00E+00 9,41E-02 9,65E+00
FW m3 0 0 5,98E-04 1,65E-03 3,77E-03 -2,29E-02
PERE = Use of renewable primary energy excluding renewable primary energy resources used as raw materials; PERM = Use of renewable primary energy resources used
as raw materials; PERT = Total use of renewable primary energy resources; PENRE = Use of non renewable primary energy excluding non-renewable primary energy
resources used as raw materials; PENRM = Use of non renewable primary energy resources used as raw materials; PENRT = Total use of non renewable primary energy
resources; SM = Use of secondary materials; RSF = Use of renewable secondary fuels; NRSF = Use of non-renewable secondary fuels; FW = Net use of fresh water
"Reading example: 9,0 E-03 = 9,0*10-3 = 0,009"
*INA Indicator Not Assessed
9 / 12
End of life - Waste
Indicator Unit A1-A3 A4 A5 B2 B3
HWD kg 4,30E-01 1,40E-03 0,00E+00 0 0
NHWD kg 4,20E+01 2,22E+00 1,96E+01 0 0
RWD kg 1,17E-02 1,74E-04 0,00E+00 0 0
Indicator Unit B4 C1 C2 C3 C4 D
HWD kg 0 0 2,90E-04 0,00E+00 1,66E+01 -4,85E-02
NHWD kg 0 0 2,71E-01 5,80E-01 1,11E-01 -3,83E+00
RWD kg 0 0 3,87E-05 0,00E+00 2,59E-05 2,35E-05
HWD = Hazardous waste disposed; NHWD = Non-hazardous waste disposed; RWD = Radioactive waste disposed
"Reading example: 9,0 E-03 = 9,0*10-3 = 0,009"
*INA Indicator Not Assessed
End of life - Output flow
Indicator Unit A1-A3 A4 A5 B2 B3
CRU kg 0,00E+00 0,00E+00 0,00E+00 0 0
MFR kg 4,97E+00 0,00E+00 2,42E+00 0 0
MER kg 0,00E+00 0,00E+00 1,67E+01 0 0
EEE MJ 0,00E+00 0,00E+00 1,18E+01 0 0
EET MJ 0,00E+00 0,00E+00 1,78E+02 0 0
Indicator Unit B4 C1 C2 C3 C4 D
CRU kg 0 0 0,00E+00 0,00E+00 0,00E+00 0,00E+00
MFR kg 0 0 0,00E+00 8,50E+00 0,00E+00 0,00E+00
MER kg 0 0 0,00E+00 2,56E+01 0,00E+00 0,00E+00
EEE MJ 0 0 0,00E+00 6,94E-01 0,00E+00 0,00E+00
EET MJ 0 0 0,00E+00 1,05E+01 0,00E+00 0,00E+00
CRU = Components for re-use; MFR = Materials for recycling; MER = Materials for energy recovery; EEE = Exported energy electrical; EET = Exported energy thermal
"Reading example: 9,0 E-03 = 9,0*10-3 = 0,009"
*INA Indicator Not Assessed
Biogenic Carbon Content
Indicator Unit At the factory gate
Biogenic carbon content in product kg C 0,00E+00
Biogenic carbon content in accompanying packaging kg C 8,13E+00
Note: 1 kg biogenic carbon is equivalent to 44/12 kg CO2
10 / 12
Additional requirements
Greenhouse gas emissions from the use of electricity in the manufacturing phase
National production mix from import, low voltage (production of transmission lines, in addition to direct emissions and losses in grid) of applied
electricity for the manufacturing process (A3).
Electricity mix Source Amount Unit
Electricity, Sweden (kWh) ecoinvent 3.6 54,94 g CO2-eq/kWh
Dangerous substances
The product contains no substances given by the REACH Candidate list.
Indoor environment
Additional Environmental Information
Key Environmental Indicators
Key environmental indicators Unit A1-A3 A4 A1-C4 A1-D
GWPtotal kg CO2 -eq 58,00 1,64 92,01 82,64
Total energy consumption MJ 2200,15 25,92 2243,90 2165,89
Amount of recycled materials % 0,09
Additional environmental impact indicators required in NPCR Part A for construction products
Indicator Unit A1-A3 A4 A5 B2 B3
GWPIOBC kg CO2 -eq 8,78E+01 1,64E+00 5,10E-01 0 0
Indicator Unit B4 C1 C2 C3 C4 D
GWPIOBC kg CO2 -eq 0 0 3,77E-01 8,50E-01 1,79E-01 -1,40E+01
GWP-IOBC: Global warming potential calculated according to the principle of instantaneous oxidation. In order to increase the transparency of biogenic carbon
contribution to climate impact, the indicator GWP-IOBC is required as it declares climate impacts calculated according to the principle of instantaneous oxidation.
GWP-IOBC is also referred to as GWP-GHG in context to Swedish public procurement legislation.
11 / 12
Bibliography
ISO 14025:2010 Environmental labels and declarations - Type III environmental declarations - Principles and procedures.
ISO 14044:2006 Environmental management - Life cycle assessment - Requirements and guidelines.
EN 15804:2012+A2:2019 Environmental product declaration - Core rules for the product category of construction products.
ISO 21930:2017 Sustainability in buildings and civil engineering works - Core rules for environmental product declarations of construction
products.
ecoinvent v3, Allocation, cut-off by classification, Swiss Centre of Life Cycle Inventories.
Iversen et al., (2021) eEPD v2021.09 Background information for EPD generator tool system verification, LCA.no Report number: 07.21
Ruud et al., (2023) EPD generator for NPCR026 Part B for Furniture - Background information for EPD generator application and LCA data,
LCA.no report number 01.23
NPCR Part A: Construction products and services. Ver. 2.0. March 2021, EPD-Norge.
NPCR 026 Part B for Furniture. Ver. 2.0 March 2022, EPD-Norge.
Program operator and publisher Phone: +47 977 22 020
The Norwegian EPD Foundation e-mail: post@epd-norge.no
Post Box 5250 Majorstuen, 0303 Oslo, Norway web: www.epd-norge.no
Owner of the declaration: Phone: 08-702 19 60
Nola Industrier Aktiebolag e-mail: anders.akesson@nola.se
Blekingegatan 26, 118 56 Stockholm web: https://nola.se/
Author of the Life Cycle Assessment Phone: +47 916 50 916
LCA.no AS e-mail: post@lca.no
Dokka 6A, 1671 Kråkerøy web: www.lca.no
Developer of EPD generator Phone: +47 916 50 916
LCA.no AS e-mail: post@lca.no
Dokka 6A, 1671 Kråkerøy web: www.lca.no
ECO Platform web: www.eco-platform.org
ECO Portal web: ECO Portal
12 / 12
