ver1 2015
ENVIRONMENTAL PRODUCT DECLARATION
in accordance with ISO 14025, ISO 21930 and EN 15804
Owner of the declaration: Con-Form Group AS
Program operator: The Norwegian EPD Foundation
Publisher: The Norwegian EPD Foundation
Declaration number: NEPD-2953-1645-EN
Registration number: NEPD-2953-1645-EN
ECO Platform reference number: -
Issue date: 05.07.2021
Valid to: 05.07.2026
Plattendekke, forspent (Strömstad)
Con-Form Group AS
www.epd-norge.no
NEPD-2953-1645-EN Plattendekke, forspent (Strömstad)
1 / 8
General information
Product: Owner of the declaration:
Plattendekke, forspent (Strömstad)
Con-Form Group AS
Contact person: Magne Aarsland
Phone: +47 93239763
e-mail: Magne.Aarsland@con-form.no
Program operator: Manufacturer:
Con-Form Group AS
The Norwegian EPD Foundation
Østensjøveien 36 0667 OSLO
Pb. 5250 Majorstuen, 0303 Oslo
Norway
Phone: +47 23 08 80 00
e-mail: post@epd-norge.no
Declaration number: Place of production:
Con-Form Strömstad AB
NEPD-2953-1645-EN Norra Båleröd 1 452 94 Strömstad
Sweden
ECO Platform reference number: Management system:
Con-Forms miljøstyringssystem er basert på ISO 14001
This declaration is based on Product Category Rules: Organisation no:
976 736 311
CEN Standard EN 15804:2012+A1:2013 serves as core PCR
NPCR 020:2018 Part B for Concrete and concrete elements
Statement of liability: Issue date: 05.07.2021
The owner of the declaration shall be liable for the underlying information and
evidence. EPD Norway shall not be liable with respect to manufacturer Valid to: 05.07.2026
information, life cycle assessment data and evidences.
Declared unit: Year of study:
1 m2 Plattendekke, forspent (Strömstad) 2020
Declared unit with option: Comparability:
EPD of construction products may not be comparable if they not comply with EN
A1,A2,A3,A4,A5
15804 and seen in a building context.
Functional unit: Development and verification of EPD:
1 m2 who are cast completed on site after installation of technical The declaration has been developed and verified using EPD tool lca.tools
installations ver EPD2020.11, developed by LCA.no AS. The EPD tool is integrated into
the company's environmental management system, and has been
approved by EPD-Norway
General information on verification of EPD from EPD tools:
Independent verification of data, other environmental information and Developer of EPD:
the declaration according to ISO 14025:2010, § 8.1.3 and § 8.1.4. Individual
third party verification of each EPD is not required when the EPD tool is i) Tore Aasen
integrated into the company's environmental management system, ii) the
procedures for use of the EPD tool are approved by EPDNorway, and iii) Reviewer of company-specific input data and EPD:
the proccess is reviewed annualy. See Appendix G of EPD-Norway's
General Programme Instructions for further information on EPD tools. Urban Holme
Verification of EPD tool: Approved:
Independent third party verification of the EPD tool, background data
Sign
and test-EPD in accordance with EPDNorway's procedures and guidelines
for verification and approval of EPD tools.
Anne Rønning, Norsus AS
(no signature required) Håkon Hauan, CEO EPD-Norge
NEPD-2953-1645-EN Plattendekke, forspent (Strömstad)
2 / 8
Product
Product description: Technical data:
Plattedekke (flooring) with pre-stressed reinforcement, for use in all types Plattendekke consists of 50 mm layer. Manufactured according to SSEN
of concrete buildings. The elements have high mechanical strength, large 13747, SSEN 13369. Concrete is produced in accordance with the
capacity and durability against climate stress. Plattendekke is used as a requirements of SS-EN-206.
starting point for the compact floor. Technical installations before final
casting on site. Weight of this type of Plattendekke is about 188kg / m2.
Product specification Market:
Plattendekke with concrete B45 M60. 1 m2 Plattendekke contains this
South-west of Sweden and eastern part of Norway (Oslo-area)
percentage distribution of sub-materials:
Reference service life, product
Materials kg % 100 year according to normal standard
Cement 30,56 16,25
Reference service life, building
Aggregate 133,71 71,11
100 year according to normal standard
Water 15,28 8,13
Chemicals 0,81 0,43
Reinforcement 5,66 3,01
Steel 2,02 1,07
Total: 188,05
LCA: Calculation rules
Declared unit: Allocation:
The allocation is made in accordance with the provisions of EN 15804.
1 m2 Plattendekke, forspent (Strömstad)
Incoming energy and water and waste production in-house is allocated
Cut-off criteria: equally among all products through mass allocation. Effects of primary
production of recycled materials is allocated to the main product in
All major raw materials and all the essential energy is included. The
which the material was used. The recycling process and transportation of
production processes for raw materials and energy flows with very small
the material is allocated to this analysis.
amounts (less than 1%) are not included. These cut-off criteria do not
apply for hazardous materials and substances.
Data quality:
Specific data for the product composition are provided by the manufacturer. They represent the production of the declared product and were collected for
EPD development in the year of study. Background data is based on registered EPDs according to EN 15804, Ostfold Research databases, ecoinvent and other
LCA databases. The data quality of the raw materials in A1 is presented in the table below.
Materials Source Data quality Year
Aggregate EcoInvent 3 Database 0
Aggregate Modified EcoInvent Database 2012
Reinforcement Østfoldforskning Database 2012
Reinforcement AENOR EPD 001-001 EPD 2015
Chemicals EPD-EFC-20150091-IAG1-EN EPD 2015
Water ecoinvent 3.4 Database 2017
Chemicals EPD-BAS-20170089-IBC1-EN EPD 2017
Steel EPD-BMG-GB-10.2 EPD 2018
Cement EPD-HCG-20190140-CAA1-EN EPD 2019
NEPD-2953-1645-EN Plattendekke, forspent (Strömstad)
3 / 8
System boundary:
Modules A1-A5 are included in the analysis. It includes all processes from extraction and production of raw materials, transport to the factory, the production
process itself. In addition, transport to the construction site (150 km) has been included in accordance with guidelines.
Final casting of concrete is not included in the declaration as the volume of this depends on several project-specific conditions.
Additional technical information:
Con-Form has established and follows its own Quality System / Production Description as a basis for the certification by Nordcerts and an Environmental
Management System based on NS-EN 14001
NEPD-2953-1645-EN Plattendekke, forspent (Strömstad)
4 / 8
LCA: Scenarios and additional technical information
The following information describe the scenarios in the different modules of the EPD.
Transport from production place to user (A4)
Capacity utilisation Fuel/Energy
Type Type of vehicle Distance km Unit Value (l/t)
(incl. return) % consumption
Truck 55,0 % Lastebil med henger, EURO 6 150 0,022606 l/tkm 3,39
Railway l/tkm
Boat l/tkm
Other Transportation l/tkm
Assembly (A5)
. Unit Value
Auxiliary kg
Water consumption m3
Electricity consumption kWh 0,5425
Other energy carriers MJ
Material loss kg
Output materials from waste treatment kg 0,1734
Dust in the air kg
VOC emissions kg
NEPD-2953-1645-EN Plattendekke, forspent (Strömstad)
5 / 8
LCA: Results
The LCA results are presented below for the declared unit defined on page 2 of the EPD document.
System boundaries (X=included, MND=module not declared, MNR=module not relevant)
Construction Beyond the
Product stage installation User stage End of life stage . system
stage bondaries
A1 A2 A3 A4 A5 B1 B2 B3 B4 B5 B6 B7 C1 C2 C3 C4 . D
X X X X X MND MND MND MND MND MND MND MND MND MND MND . MND
Environmental impact
Parameter Unit A1 A2 A3 A4 A5
GWP kg CO 2 -eq 3,15E+01 1,44E+00 2,90E+00 2,34E+00 2,31E-01
ODP kg CFC11 -eq 9,40E-07 2,77E-07 6,65E-07 4,80E-07 1,69E-08
POCP kg C 2H 4-eq 5,35E-03 2,27E-04 4,44E-04 3,65E-04 3,10E-05
AP kg SO 2 -eq 9,00E-02 5,15E-03 9,17E-03 6,03E-03 7,97E-04
EP kg PO 3- -eq 1,83E-02 8,78E-04 1,61E-03 8,32E-04 1,70E-04
4
ADPM kg Sb -eq -3,74E-05 2,86E-06 2,97E-06 5,56E-06 3,66E-07
ADPE MJ 1,35E+02 2,24E+01 3,68E+01 3,83E+01 2,13E+00
GWP Global warming potential; ODP Depletion potential of the stratospheric ozone layer; POCP Formation potential of tropospheric photochemical oxidants;
AP Acidification potential of land and water; EP Eutrophication potential; ADPM Abiotic depletion potential for non fossil resources; ADPE Abiotic depletion
potential for fossil resources
Reading example: 9,0 E-03 = 9,0*10-3 = 0,009
*INA Indicator Not Assessed
waR slairetam tropsnarT gnirutcafunaM tropsnarT ylbmessA esU ecnanetniaM riapeR tnemecalpeR tnemhsibrufeR lanoitarepO ygrene esu lanoitarepO esu
retaw
-eD noitcurtsnoc noitilomed tropsnarT etsaW gnissecorp lasopsiD -yrevoceR-esueR -gnilcyceR laitnetop
NEPD-2953-1645-EN Plattendekke, forspent (Strömstad)
6 / 8
Resource use
Parameter Unit A1 A2 A3 A4 A5
RPEE MJ 4,35E+01 4,23E-01 1,40E+01 6,97E-01 3,35E+00
RPEM MJ 6,39E-01 0,00E+00 0,00E+00 0,00E+00 0,00E+00
TPE MJ 4,87E+01 4,23E-01 1,40E+01 6,97E-01 3,71E+00
NRPE MJ 1,49E+02 2,32E+01 6,40E+01 3,95E+01 2,20E+00
NRPM MJ 1,43E+00 0,00E+00 0,00E+00 0,00E+00 0,00E+00
TRPE MJ 1,64E+02 2,32E+01 6,40E+01 3,95E+01 3,24E+00
SM kg 9,64E+00 0,00E+00 0,00E+00 0,00E+00 1,84E-01
RSF MJ 8,19E+00 0,00E+00 1,18E-02 0,00E+00 3,85E-04
NRSF MJ 1,80E+01 0,00E+00 0,00E+00 0,00E+00 0,00E+00
W m3 4,31E+01 5,47E-03 4,69E-02 9,36E-03 1,48E-01
RPEE Renewable primary energy resources used as energy carrier; RPEM Renewable primary energy resources used as raw materials; TPE Total use of renewable
primary energy resources; NRPE Non renewable primary energy resources used as energy carrier; NRPM Non renewable primary energy resources used as
materials; TRPE Total use of non renewable primary energy resources; SM Use of secondary materials; RSF Use of renewable secondary fuels; NRSF Use of non
renewable secondary fuels; W Use of net fresh water
Reading example: 9,0 E-03 = 9,0*10-3 = 0,009
*INA Indicator Not Assessed
End of life - Waste
Parameter Unit A1 A2 A3 A4 A5
HW kg 1,33E-01 1,34E-05 1,18E-02 2,11E-05 1,03E-02
NHW kg 5,93E+00 1,79E+00 2,01E+00 3,61E+00 4,47E-01
RW kg INA* INA* INA* INA* INA*
HW Hazardous waste disposed; NHW Non hazardous waste disposed; RW Radioactive waste disposed
Reading example: 9,0 E-03 = 9,0*10-3 = 0,009
*INA Indicator Not Assessed
End of life - Output flow
Parameter Unit A1 A2 A3 A4 A5
CR kg 0,00E+00 0,00E+00 0,00E+00 0,00E+00 0,00E+00
MR kg 9,64E-01 0,00E+00 7,30E-01 0,00E+00 1,77E-03
MER kg 0,00E+00 0,00E+00 1,89E-01 0,00E+00 1,60E-01
EEE MJ INA* INA* INA* INA* INA*
ETE MJ INA* INA* INA* INA* INA*
CR Components for reuse; MR Materials for recycling; MER Materials for energy recovery; EEE Exported electric energy; ETE Exported thermal energy
Reading example: 9,0 E-03 = 9,0*10-3 = 0,009
*INA Indicator Not Assessed
NEPD-2953-1645-EN Plattendekke, forspent (Strömstad)
7 / 8
Additional Norwegian requirements
Greenhouse gas emissions from the use of electricity in the manufacturing phase
National production mix from import, low voltage (production of transmission lines, in addition to direct emissions and losses in grid) of applied electricity for
the manufacturing process (A3).
Electricity mix Data source Amount Unit
El-mix, Sweden (kWh) ecoinvent 3.4 Alloc Rec 42,67 g CO2-ekv/kWh
Dangerous substances
The product contains no substances given by the REACH Candidate list or the Norwegian priority list.
Indoor environment
No impact on indoor climate
Bibliography
ISO 14025:2010 Environmental labels and declarations - Type III environmental declarations - Principles and procedures.
ISO 14044:2006 Environmental management - Life cycle assessment - Requirements and guidelines.
EN 15804:2012+A1:2013 Environmental product declaration - Core rules for the product category of construction products.
ISO 21930:2017 Sustainability in buildings and civil engineering works - Core rules for environmental product declarations of construction products.
ecoinvent v3, Allocation, cut-off by classification, Swiss Centre of Life Cycle Inventories.
Iversen et al., (2018) eEPD v3.0 - Background information for EPD generator system. LCA.no report number 04.18
Vold, M. og Edvardsen, T. (2014) EPD-generator for betongindustrien, bakgrunnsinformasjon for verifisering, OR 04.14.
NPCR Part A: Construction products and services. Ver. 1.0. April 2017, EPD-Norge.
NPCR 020 Part B for Concrete and concrete elements. Ver. 2.0 October 2018, EPD-Norge.
Program operator and publisher Phone: +47 23 08 80 00
The Norwegian EPD Foundation e-mail: post@epd-norge.no
Post Box 5250 Majorstuen, 0303 Oslo,Norway web: www.epd-norge.no
Owner of the declaration Phone: +47 93239763
Con-Form Group AS e-mail: Magne.Aarsland@con-form.no
Østensjøveien 36 0667 OSLO web: www.con-form.no
Author of the Life Cycle Assessment Phone: +47 69 35 11 00
Østfoldforskning AS e-mail: post@ostfoldforskning.no
Stadion 4 1671 Kråkerøy web: www.ostfoldforskning.no
Developer of EPD generator Phone: +47 916 50 916
LCA.no AS e-mail: post@lca.no
Dokka 1C,1671 Kråkerøy web: www.lca.no
NEPD-2953-1645-EN Plattendekke, forspent (Strömstad)
8 / 8
