Environmental product declaration
in accordance with ISO 14025 and EN 15804+A2
MC100X50-1HV
Owner of the declaration: Program operator:
Maxeta AS The Norwegian EPD Foundation
Product: Declaration number:
MC100X50-1HV
NEPD-8086-7779-EN
Declared unit:
Registration number:
1 m
NEPD-8086-7779-EN
This declaration is based on Product Category Rules:
CEN Standard EN 15804:2012+A2:2019 serves as core Issue date: 14.11.2024
PCR
Valid to: 14.11.2029
The Norwegian EPD Foundation NPCR 028:2020 Part B for Cable pipes
EPD software:
LCAno EPD generator ID: 559640
1 / 11
General information
Product Owner of the declaration:
MC100X50-1HV Maxeta AS
Contact person: Eivind Portaas Walstad
Phone:
e-mail: maxeta@maxeta.no
Program operator: Manufacturer:
The Norwegian EPD Foundation Maxeta AS
Post Box 5250 Majorstuen, 0303 Oslo, Norway Amtmand Aallsgate 89
Phone: +47 977 22 020 3716 Skien, Norway
web: www.epd-norge.no
Declaration number: Place of production:
Maxeta AS production site (Norway)
NEPD-8086-7779-EN
Gaustadvegen 136
2240 Magnor, Norway
This declaration is based on Product Category Rules: Management system:
CEN Standard EN 15804:2012+A2:2019 serves as core PCR
NPCR 028:2020 Part B for Cable pipes
Statement of liability: Organisation no:
The owner of the declaration shall be liable for the underlying 864 425 402
information and evidence. EPD Norway shall not be liable with respect
to manufacturer information, life cycle assessment data and
evidences.​
Declared unit: Issue date:
1 m MC100X50-1HV 14.11.2024
Declared unit with option: Valid to:
A1,A2,A3,A4,A5,C1,C2,C3,C4,D 14.11.2029
Year of study:
2023
Functional unit: Comparability:
1 m of MC100X50-1HV, used for protection of electrical cables in EPD of construction products may not be comparable if they not
trenches over a specific lifetime, including waste treatment at end-of- comply with EN 15804 and seen in a building context.
life.
General information on verification of EPD from EPD tools: Development and verification of EPD:
Independent verification of data, other environmental information The declaration is created using EPD tool lca.tools ver EPD2022.03,
and the declaration according to ISO 14025:2010, § 8.1.3 and § 8.1.4. developed by LCA.no. The EPD tool is integrated in the company's
Verification of each EPD is made according to EPD-Norway’s management system, and has been approved by EPD Norway.
guidelines for verification and approval requiring that tools are i)
integrated into the company's environmental management system, ii) Developer of EPD: Konrad Muszynski
the procedures for use of the EPD tool are approved by EPD-Norway,
Reviewer of company-specific input data and EPD:​ Nathaniel Kittilsen
and iii) the process is reviewed annually by an independent third
Aale
party verifier. See Appendix G of EPD-Norway's General Programme
Instructions for further information on EPD tools
Verification of EPD tool: Approved:
Independent third party verification of the EPD tool, background data
and test-EPD in accordance with EPDNorway's procedures and
guidelines for verification and approval of EPD tools. Approval
number: NEPDT49.
Third party verifier:
Vito D’Incognito, Take Care International
(no signature required)
2 / 11
Product
Product description:
MAXCOMBI 100 Series
The system uses fixing frames for equipment installation. It is a universal and flexible channel solution for materials with 45 mm and 60 mm
attachment points. It is suitable for small to medium installations where the capacity needs for the number of cables are somewhat limited. The
profile is available in two depth options: 65 mm and 50 mm.
Product specification
Aluminium Cable Trunking
The trunking has good capacity and offers all the advantages for possible installation of standard recessed equipment and 45 mm equipment with
mounting frames.
Materials kg %
Powder coating 0,10 8,00
Metal - Aluminium 1,15 92,00
Total 1,25 100,00
Technical data:
Aluminium Cable Trunking
100x50mm with 77mm cover
General information: https://maxeta.no/produkt/maxcombi-100/?
attribute_pa_farge3=hvit&attribute_pa_breddemm=100&attribute_pa_hoydemm0=50&attribute_pa_standardlengdem0=3&sku=MC100X50-
1HV
Market:
Norway/Nordics
Reference service life, product
30 years
Reference service life, building or construction works
LCA: Calculation rules
Declared unit:
1 m MC100X50-1HV
Cut-off criteria:
All major raw materials and all the essential energy is included. The production processes for raw materials and energy flows with very small
amounts (less than 1%) are not included. These cut-off criteria do not apply for hazardous materials and substances.
Allocation:
The allocation is made in accordance with the provisions of EN 15804:2012+A2:2019. Incoming energy and water and waste production in-house
is allocated equally among all products through mass allocation. Effects of primary production of recycled materials is allocated to the main
product in which the material was used. The recycling process and transportation of the material is allocated to this analysis.
Data quality:
Specific data for the product composition are provided by the manufacturer. The data represent the production of the declared product and were
collected for EPD development in the year of study. Background data is based on EPDs according to EN 15804 and different LCA databases. The
data quality of the raw materials in A1 is presented in the table below.
Materials Source Data quality Year
Metal - Aluminium S-P-07377 EPD 2021
Powder coating Ecoinvent 3.6 Database 2019
3 / 11
System boundaries (X=included, MND=module not declared, MNR=module not relevant)
Construction Beyond the system
Product stage Use stage End of life stage
installation stage boundaries
A1 A2 A3 A4 A5 B1 B2 B3 B4 B5 B6 B7 C1 C2 C3 C4 D
X X X X X MND MND MND MND MND MND MND X X X X X
System boundary:
Additional technical information:
waR slairetam tropsnarT gnirutcafunaM tropsnarT ylbmessA e​sU ecnanetniaM riapeR tnemecalpeR tnemhsibrufeR lanoitarepO ygrene esu lanoitarepO esu retaw -eD noitcurtsnoc noitilomed tropsnarT etsaW gnissecorp lasopsiD -yrevoceR-esueR laitnetop-gnilcyceR
4 / 11
LCA: Scenarios and additional technical information
The following information describe the scenarios in the different modules of the EPD.
Module A4 = 300 km considered as the average transport between warehouse to customer
Modules A5 = 1 % product losses during installation are estimated by the company. No energy use has been quantified since installation in
buildings is often done by manual labour. Use of portable electrical devices (e.g., drill) usually have low energy requirements falling under the cut-
off criterion of 1%.
Module C1 = de-construction in buildings is often done by manual labour. Use of portable electrical devices (e.g., drill) usually have low energy
requirements falling under the cut-off criterion of 1%.
Module C2 = 85 km is considered the average default transport from demolition to waste treatment facility
Modules C3 and C4 = Waste treatment of the product follows the default values provided in EN 50693, Product Category Rules for life cycle
assessments of electronic and electrical products and systems, table G.4. This table specified how different types of raw materials used in A1 will
likely be treated during the end-of-life of the product. Waste treatments in C3 include material recycling and incineration with and without energy
recovery and fly ash extraction. Disposal in C4 consist of landfilling of different waste fractions and of ashes.
Module D = The recyclability of metals and plastics allows the producers a credit for the net scrap that is produced at the end of a product’s life.
The benefits from recycling of net scrap are described in formula from EN 15804:2012+A2:2019. Substitution of heat and electricity generated by
the incineration with energy recovery of plastics is also calculated in module D.
Capacity utilisation Value
Transport from production place to user (A4) Distance (km) Fuel/Energy Consumption Unit
(incl. return) % (Liter/tonne)
Truck, 16-32 tonnes, EURO 5 (km) 36,7 % 300 0,044 l/tkm 13,20
Assembly (A5) Unit Value
Product loss during installation (percentage of
Units/DU 0,01
cable pipe)
Capacity utilisation Value
Transport to waste processing (C2) Distance (km) Fuel/Energy Consumption Unit
(incl. return) % (Liter/tonne)
Truck, 16-32 tonnes, EURO 5 (km) 36,7 % 85 0,044 l/tkm 3,74
Waste processing (C3) Unit Value
Aluminium to recycling (kg) kg 0,81
Disposal (C4) Unit Value
Landfilling of aluminium (kg) kg 0,35
Landfilling of hazardous waste (kg) kg 0,10
Benefits and loads beyond the system
Unit Value
boundaries (D)
Substitution of primary aluminium with net scrap
kg 0,81
(kg)
5 / 11
LCA: Results
The LCA results are presented below for the declared unit defined on page 2 of the EPD document.
Environmental impact
Indicator Unit A1 A2 A3 A4 A5 C1 C2 C3 C4 D
GWP-total
kg CO2 -
6,41E+00 1,11E-01 2,59E-02 6,26E-02 6,64E-02 0 1,77E-02 0,00E+00 2,65E-02 -7,32E+00
eq
GWP-fossil
kg CO2 -
6,28E+00 1,11E-01 2,52E-02 6,25E-02 6,50E-02 0 1,77E-02 0,00E+00 2,62E-02 -7,15E+00
eq
GWP-biogenic
kg CO2 -
1,23E-01 4,52E-05 6,04E-04 2,55E-05 1,24E-03 0 7,22E-06 0,00E+00 1,87E-05 -3,29E-02
eq
GWP-luluc
kg CO2 -
1,01E-02 3,88E-05 9,27E-05 2,19E-05 1,05E-04 0 6,19E-06 0,00E+00 1,90E-04 -1,36E-01
eq
kg
ODP CFC11 - 6,57E-07 2,53E-08 1,81E-09 1,43E-08 7,01E-09 0 4,04E-09 0,00E+00 2,46E-09 -6,03E-07
eq
mol H+
AP 3,96E-02 4,53E-04 1,87E-04 2,56E-04 4,07E-04 0 7,24E-05 0,00E+00 1,38E-04 -4,84E-02
-eq
EP-FreshWater kg P -eq 1,30E-04 8,71E-07 1,83E-06 4,91E-07 1,34E-06 0 1,39E-07 0,00E+00 1,04E-06 -2,76E-04
EP-Marine kg N -eq 6,05E-03 1,34E-04 2,19E-05 7,58E-05 6,32E-05 0 2,15E-05 0,00E+00 3,39E-05 -6,11E-03
mol N -
EP-Terrestial 6,35E-02 1,49E-03 2,79E-04 8,38E-04 6,65E-04 0 2,37E-04 0,00E+00 3,70E-04 -6,72E-02
eq
kg
POCP NMVOC 1,92E-02 4,55E-04 7,70E-05 2,57E-04 2,02E-04 0 7,27E-05 0,00E+00 1,50E-04 -2,27E-02
-eq
ADP- kg Sb-
1,76E-05 3,00E-06 1,67E-06 1,69E-06 2,42E-07 0 4,80E-07 0,00E+00 1,61E-07 1,10E-05
minerals&metals1 eq
ADP-fossil1 MJ 1,13E+02 1,67E+00 3,56E-01 9,43E-01 1,16E+00 0 2,67E-01 0,00E+00 3,48E-01 -9,09E+01
WDP1 m3 5,18E+01 1,59E+00 5,09E+01 8,99E-01 1,08E+00 0 2,55E-01 0,00E+00 3,13E+00 -4,10E+03
GWP-total = Global Warming Potential total; GWP-fossil = Global Warming Potential fossil fuels; GWP-biogenic = Global Warming Potential biogenic; GWP-luluc =
Global Warming Potential land use and land use change; ODP = Depletion potential of the stratospheric ozone layer; AP = Acidification potential, Accumulated
Exceedance; EP-freshwater = Eutrophication potential, fraction of nutrients reaching freshwater end compartment: EP-marine = Eutrophication potential, fraction of
nutrients reaching marine end compartment; EP-terrestrial = Eutrophication potential, Accumulated Exceedance; POCP = Formation potential of tropospheric ozone;
ADP-minerals&metals = Abiotic depletion potential for non-fossil resources; ADP-fossil = Abiotic depletion for fossil resources potential; WDP = Water (user)
deprivation potential, deprivation-weighted water consumption
"Reading example: 9,0 E-03 = 9,0*10-3 = 0,009"
*INA Indicator Not Assessed
1. The results of this environmental impact indicator shall be used with care as the uncertainties on these results are high or as there is limited experienced with the
indicator
Remarks to environmental impacts
6 / 11
Additional environmental impact indicators
Indicator Unit A1 A2 A3 A4 A5 C1 C2 C3 C4 D
PM Disease incidence 3,07E-08 7,98E-09 1,37E-09 4,50E-09 4,70E-10 0 1,28E-09 0,00E+00 2,48E-09 -4,99E-07
IRP2 kgBq U235 -eq 3,64E-02 7,31E-03 5,65E-03 4,12E-03 5,46E-04 0 1,17E-03 0,00E+00 1,11E-03 -3,95E-01
ETP-fw1 CTUe 1,74E+01 1,23E+00 1,37E+00 6,94E-01 2,35E+00 0 1,97E-01 0,00E+00 2,14E+02 -1,08E+02
HTP-c1 CTUh 1,36E-09 0,00E+00 7,30E-11 0,00E+00 1,50E-11 0 0,00E+00 0,00E+00 1,05E-10 -1,81E-08
HTP-nc1 CTUh 1,07E-08 1,33E-09 1,71E-09 7,50E-10 1,53E-10 0 2,13E-10 0,00E+00 8,39E-10 -2,11E-07
SQP1 dimensionless 3,36E+00 1,15E+00 1,63E-01 6,50E-01 6,12E-02 0 1,84E-01 0,00E+00 7,93E-01 -7,77E-01
PM = Particulate Matter emissions; IRP = Ionizing radiation – human health; ETP-fw = Eco toxicity – freshwater; HTP-c = Human toxicity – cancer effects; HTP-nc =
Human toxicity – non cancer effects; SQP = Potential Soil Quality Index (dimensionless)
"Reading example: 9,0 E-03 = 9,0*10-3 = 0,009"
*INA Indicator Not Assessed
1. The results of this environmental impact indicator shall be used with care as the uncertainties on these results are high or as there is limited experienced with the
indicator
2. This impact category deals mainly with the eventual impact of low dose ionizing radiation on human health of the nuclear fuel cycle. It does not consider effects due
to possible nuclear accidents, occupational exposure nor due to radioactive waste disposal in underground facilities. Potential ionizing radiation from the soil, from
radon and from some construction materials is also not measured by this indicator.
7 / 11
Resource use
Indicator Unit A1 A2 A3 A4 A5 C1 C2 C3 C4 D
PERE MJ 9,50E+01 2,36E-02 3,70E+00 1,33E-02 9,89E-01 0 3,77E-03 0,00E+00 9,84E-02 -3,29E+01
PERM MJ 0,00E+00 0,00E+00 0,00E+00 0,00E+00 0,00E+00 0 0,00E+00 0,00E+00 0,00E+00 0,00E+00
PERT MJ 9,50E+01 2,36E-02 3,70E+00 1,33E-02 9,89E-01 0 3,77E-03 0,00E+00 9,84E-02 -3,29E+01
PENRE MJ 1,13E+02 1,67E+00 3,56E-01 9,43E-01 1,16E+00 0 2,67E-01 0,00E+00 3,49E-01 -9,09E+01
PENRM MJ 0,00E+00 0,00E+00 0,00E+00 0,00E+00 0,00E+00 0 0,00E+00 0,00E+00 0,00E+00 0,00E+00
PENRT MJ 1,13E+02 1,67E+00 3,56E-01 9,43E-01 1,16E+00 0 2,67E-01 0,00E+00 3,49E-01 -9,09E+01
SM kg 0,00E+00 0,00E+00 0,00E+00 0,00E+00 2,16E-05 0 0,00E+00 0,00E+00 2,16E-03 0,00E+00
RSF MJ 4,80E-02 8,44E-04 3,66E-03 4,76E-04 5,35E-04 0 1,35E-04 0,00E+00 5,06E-04 -1,34E-02
NRSF MJ 1,13E-02 3,01E-03 7,97E-03 1,70E-03 4,27E-04 0 4,82E-04 0,00E+00 1,87E-02 4,84E-02
FW m3 6,22E-01 1,76E-04 3,96E-02 9,93E-05 6,62E-03 0 2,81E-05 0,00E+00 2,75E-04 -1,80E-01
PERE = Use of renewable primary energy excluding renewable primary energy resources used as raw materials; PERM = Use of renewable primary energy resources used
as raw materials; PERT = Total use of renewable primary energy resources; PENRE = Use of non renewable primary energy excluding non-renewable primary energy
resources used as raw materials; PENRM = Use of non renewable primary energy resources used as raw materials; PENRT = Total use of non renewable primary energy
resources; SM = Use of secondary materials; RSF = Use of renewable secondary fuels; NRSF = Use of non-renewable secondary fuels; FW = Net use of fresh water
"Reading example: 9,0 E-03 = 9,0*10-3 = 0,009"
*INA Indicator Not Assessed
8 / 11
End of life - Waste
Indicator Unit A1 A2 A3 A4 A5 C1 C2 C3 C4 D
HWD kg 3,91E-02 8,53E-05 2,08E-04 4,81E-05 1,52E-03 0 1,36E-05 0,00E+00 1,13E-01 3,01E-02
NHWD kg 4,59E+00 7,99E-02 2,36E-02 4,50E-02 5,09E-02 0 1,28E-02 0,00E+00 3,50E-01 -2,08E+00
RWD kg 1,89E-02 1,14E-05 2,96E-06 6,43E-06 1,89E-04 0 1,82E-06 0,00E+00 7,98E-07 -3,72E-04
HWD = Hazardous waste disposed; NHWD = Non-hazardous waste disposed; RWD = Radioactive waste disposed
"Reading example: 9,0 E-03 = 9,0*10-3 = 0,009"
*INA Indicator Not Assessed
End of life - Output flow
Indicator Unit A1 A2 A3 A4 A5 C1 C2 C3 C4 D
CRU kg 0,00E+00 0,00E+00 0,00E+00 0,00E+00 0,00E+00 0 0,00E+00 0,00E+00 0,00E+00 0,00E+00
MFR kg 0,00E+00 0,00E+00 1,71E-03 0,00E+00 8,07E-03 0 0,00E+00 8,05E-01 0,00E+00 0,00E+00
MER kg 0,00E+00 0,00E+00 1,07E-03 0,00E+00 1,07E-05 0 0,00E+00 0,00E+00 0,00E+00 0,00E+00
EEE MJ 0,00E+00 0,00E+00 8,05E-04 0,00E+00 8,05E-06 0 0,00E+00 0,00E+00 0,00E+00 0,00E+00
EET MJ 0,00E+00 0,00E+00 1,22E-02 0,00E+00 1,22E-04 0 0,00E+00 0,00E+00 0,00E+00 0,00E+00
CRU = Components for re-use; MFR = Materials for recycling; MER = Materials for energy recovery; EEE = Exported energy electrical; EET = Exported energy thermal
"Reading example: 9,0 E-03 = 9,0*10-3 = 0,009"
*INA Indicator Not Assessed
Biogenic Carbon Content
Indicator Unit At the factory gate
Biogenic carbon content in product kg C 0,00E+00
Biogenic carbon content in accompanying packaging kg C 0,00E+00
Note: 1 kg biogenic carbon is equivalent to 44/12 kg CO2
9 / 11
Additional requirements
Greenhouse gas emissions from the use of electricity in the manufacturing phase
National production mix from import, low voltage (production of transmission lines, in addition to direct emissions and losses in grid) of applied
electricity for the manufacturing process (A3).
Electricity mix Source Amount Unit
Electricity, Norway (kWh) ecoinvent 3.6 24,33 g CO2-eq/kWh
Dangerous substances
The product contains no substances given by the REACH Candidate list.
Indoor environment
Additional Environmental Information
Additional environmental impact indicators required in NPCR Part A for construction products
Indicator Unit A1 A2 A3 A4 A5 C1 C2 C3 C4 D
GWPIOBC kg CO2 -eq 6,29E+00 1,11E-01 2,58E-02 6,26E-02 6,52E-02 0 1,77E-02 0,00E+00 2,74E-02 -6,98E+00
GWP-IOBC: Global warming potential calculated according to the principle of instantaneous oxidation. In order to increase the transparency of biogenic carbon​
contribution to climate impact, the indicator GWP-IOBC is required as it declares climate impacts calculated according to the principle of instantaneous oxidation.​
GWP-IOBC is also referred to as GWP-GHG in context to Swedish public procurement legislation.
10 / 11
Bibliography
ISO 14025:2010. Environmental labels and declarations - Type III environmental declarations - Principles and procedures. International
Organization for Standardization.
ISO 14044:2006. Environmental management - Life cycle assessment - Requirements and guidelines. International Organization for
Standardization.
EN 15804:2012+A2:2019. Environmental product declaration - Core rules for the product category of construction products. European
Committee for Standardization.
ISO 21930:2017. Sustainability in buildings and civil engineering works - Core rules for environmental product declarations of construction
products. International Organization for Standardization.
EN 50693:2019. Product category rules for life cycle assessments of electronic and electrical products and systems. European Committee for
Standardization.
Ecoinvent v3, 2019. Allocation, cut-off by classification. Swiss Centre of Life Cycle Inventories.
Iversen et al., (2021). eEPD v2021.09, background information for EPD generator tool system verification, LCA.no. Report number: 07.21. System
verification report.
Philis et al., (2022). EPD generator for NPCR 028 part B for cable pipes, background information for EPD generator application and LCA data,
LCA.no Report number: 06.22. PCR verification report.
EPD Norway (2022). NPCR Part A: Construction products and services. The Norwegian EPD foundation. Version 2.0 published 24.03.2021.
EPD Norway (2022). NPCR 027 Part B for cable pipes. The Norwegian EPD foundation. Version 2.0 published 31.03.2022.
Program operator and publisher Phone: +47 977 22 020
The Norwegian EPD Foundation e-mail: post@epd-norge.no
Post Box 5250 Majorstuen, 0303 Oslo, Norway web: www.epd-norge.no
Owner of the declaration: Phone:
Maxeta AS e-mail: maxeta@maxeta.no
Amtmand Aallsgate 89, 3716 Skien web:
Author of the Life Cycle Assessment Phone: +47 916 50 916
LCA.no AS e-mail: post@lca.no
Dokka 6A, 1671 Kråkerøy web: www.lca.no
Developer of EPD generator Phone: +47 916 50 916
LCA.no AS e-mail: post@lca.no
Dokka 6A, 1671 Kråkerøy web: www.lca.no
ECO Platform web: www.eco-platform.org
ECO Portal web: ECO Portal
11 / 11
