Environmental product declaration
in accordance with ISO 14025 and EN 15804+A2
VI Kooltherm Uddevalla Biobetong 2
Owner of the declaration: Program operator:
Heidelberg Materials Precast Contiga AB – Concrete The Norwegian EPD Foundation
Product: Declaration number:
VI Kooltherm Uddevalla Biobetong 2
Registration number:
Declared unit:
1 tonne Issue date:
This declaration is based on Product Category Rules: Valid to:
CEN Standard EN 15804:2012+A2:2019 serves as core
EPD software:
PCR
The Norwegian EPD Foundation LCAno EPD generator ID: 230457
NPCR 020:2021 Part B for Concrete and concrete
elements
1 / 12
General information
Product Owner of the declaration:
VI Kooltherm Uddevalla Biobetong 2 Heidelberg Materials Precast Contiga AB – Concrete
Contact person: Håvard Nyman
Phone: +46 0522 636333
e-mail: Havard.Nyman@contiga.se
Program operator: Manufacturer:
The Norwegian EPD Foundation Heidelberg Materials Precast Contiga AB – Concrete
Post Box 5250 Majorstuen, 0303 Oslo, Norway Kasenabbevägen 11A,
Phone: +47 977 22 020 1662 451 91 Uddevalla, Sverige, Sweden
web: www.epd-norge.no
Declaration number: Place of production:
Uddevalla, Heidelberg Materials Precast Contiga AB
, Sweden
This declaration is based on Product Category Rules: Management system:
CEN Standard EN 15804:2012+A2:2019 serves as core PCR Holds a local environmental diploma and is certified for ISO45001,
NPCR 020:2021 Part B for Concrete and concrete elements 14001 and 9001
Statement of liability: Organisation no:
The owner of the declaration shall be liable for the underlying 556270-5979
information and evidence. EPD Norway shall not be liable with respect
to manufacturer information, life cycle assessment data and
evidences.​
Declared unit: Issue date:
1 tonne VI Kooltherm Uddevalla Biobetong 2
Declared unit with option: Valid to:
A1,A2,A3,A4,A5,C1,C2,C3,C4,D
Year of study:
2022
Functional unit: Comparability:
EPD of construction products may not be comparable if they not
comply with EN 15804 and seen in a building context.
General information on verification of EPD from EPD tools: Development and verification of EPD:
Independent verification of data, other environmental information The declaration is created using EPD tool lca.tools ver EPD2022.03,
and the declaration according to ISO 14025:2010, § 8.1.3 and § 8.1.4. developed by LCA.no. The EPD tool is integrated in the company's
Verification of each EPD is made according to EPD-Norway’s management system, and has been approved by EPD Norway.
guidelines for verification and approval requiring that tools are i) NEPDT03
integrated into the company's environmental management system, ii)
the procedures for use of the EPD tool are approved by EPD-Norway, Developer of EPD: Alexander Noré
and iii) the process is reviewed annually by an independent third
Reviewer of company-specific input data and EPD:​ Håvard Nyman
party verifier. See Appendix G of EPD-Norway's General Programme
Instructions for further information on EPD tools
Verification of EPD tool: Approved:
Independent third party verification of the EPD tool, background data
and test-EPD in accordance with EPDNorway's procedures and
guidelines for verification and approval of EPD tools.
Håkon Hauan, CEO EPD-Norge
Third party verifier:
Jane Anderson, Construction LCA Ltd
(no signature required)
2 / 12
Product
Product description:
A half-sandwich wall panel, combining a robust concrete layer and a layer of Kooltherm insulation, usually used as an exterior wall, offers a durable
and energy-efficient solution for modern construction. They are manufactured in different thicknesses depending on the desired function. Theese
walls are casted on horizontal mold tables with one side that is counter-molded, down in form and on side with mounted insulation, up in form.
The concrete provides structural strength and resilience, while the Kooltherm delivers excellent thermal insulation. This prefabricated unit
streamlines the building process, ensuring quick installation and airtight performance, making it ideal for a variety of architectural applications
where efficiency and longevity are paramount.
Concrete walls are 100% recyclable and enable fast, cost-effective and rational progress in the construction project.
Product specification
Materials kg %
Additives 69,77 6,98
Aggregate 740,00 74,00
Cement 90,29 9,03
Chemical 2,40 0,24
Insulation 14,36 1,44
Metal - Steel 29,29 2,93
Water 53,89 5,39
Total 1000,00
Technical data:
The declared element is 1 ton of insulated concrete wall that is a total of 300mm thick. A 150mm thick layer of concrete in the quality C35/45, w/c
ratio 0.50, and a 150mm thick layer of Kooltherm. The declared ton includes an average amount of reinforcement of 27.36kg/ton and an average
amount of cast in materials of 1.93kg/ton. The declared unit also applies to a wide range of dimensions with an average amount of reinforcement
and cast in materials.
Cement is Heidelberg Materials Bascement CEM II 42.5 R. See EPD-HCG-20210157-CAA1-EN
Concrete strength C35/45.
Exposure classes up to XC4-XF3.
Life length class up to L100 (100 years).
More technical data and information about load capacitys for the different wall dimensions is available at Heidelberg Materials Precast Contiga's
concrete factory in Uddevalla
Market:
Sweden
Reference service life, product
Lifetime depends on exposure class. Interior walls in exposure class XC0 have no limitation in service life
Reference service life, building or construction works
More than 50 years
LCA: Calculation rules
Declared unit:
1 tonne VI Kooltherm Uddevalla Biobetong 2
Cut-off criteria:
All major raw materials and all the essential energy is included. The production processes for raw materials and energy flows with very small
amounts (less than 1%) are not included. These cut-off criteria do not​ apply for hazardous materials and substances.
Allocation:
The allocation is made in accordance with the provisions of EN 15804. Incoming energy and water and waste production in-house is allocated
equally among all products through mass allocation. Effects of primary production of recycled materials is allocated to the main product in which
the material was used. The recycling process and transportation of the material is allocated to this analysis.
Data quality:
Specific data for the product composition are provided by the manufacturer. The data represent the production of the declared product and were
collected for EPD development in the year of study. Background data is based on EPDs according to EN 15804 and different LCA databases. The
data quality of the raw materials in A1 is presented in the table below.
3 / 12
Materials Source Data quality Year
Additives Supplier EPD 2022
Aggregate ecoinvent 3.6 Database 2019
Cement EPD-HCG-20210157-CAA1-EN EPD 2021
Chemical EPD-EFC-20210198-IBG1-EN EPD 2021
Insulation EPD-KSI-20210046-CBA2-EN EPD 2021
Metal - Steel Ecoinvent 3.6 Database 2019
Water ecoinvent 3.6 Database 2019
4 / 12
System boundaries (X=included, MND=module not declared, MNR=module not relevant)
Construction Beyond the system
Product stage Use stage End of life stage
installation stage boundaries
A1 A2 A3 A4 A5 B1 B2 B3 B4 B5 B6 B7 C1 C2 C3 C4 D
X X X X X MND MND MND MND MND MND MND X X X X X
System boundary:
Additional technical information:
The product can be recycled by crushing
waR slairetam tropsnarT gnirutcafunaM tropsnarT ylbmessA e​sU ecnanetniaM riapeR tnemecalpeR tnemhsibrufeR lanoitarepO ygrene esu lanoitarepO esu retaw -eD noitcurtsnoc noitilomed tropsnarT etsaW gnissecorp lasopsiD -yrevoceR-esueR laitnetop-gnilcyceR
5 / 12
LCA: Scenarios and additional technical information
The following information describe the scenarios in the different modules of the EPD.
Capacity utilisation Value
Transport from production place to user (A4) Distance (km) Fuel/Energy Consumption Unit
(incl. return) % (Liter/tonne)
Truck, over 32 tonnes, EURO 6 (km) 53,3 % 85 0,023 l/tkm 1,96
Assembly (A5) Unit Value
Diesel (L) L/DU 0,87
De-construction demolition (C1) Unit Value
Demolition of building per kg of cement-based
kg/DU 970,70
product, C1 (kg)
Demolition of building per kg of steel, C1 (kg) kg/DU 29,30
Diesel (L) L/DU 0,87
Capacity utilisation Value
Transport to waste processing (C2) Distance (km) Fuel/Energy Consumption Unit
(incl. return) % (Liter/tonne)
Truck, over 32 tonnes, EURO 6 (km) 53,3 % 85 0,023 l/tkm 1,96
Waste processing (C3) Unit Value
Materials to recycling (kg) kg 19,63
Waste treatment of cement-based product after
kg 660,08
demolition (kg
Disposal (C4) Unit Value
Waste, concrete sludge, rest concrete, to disposal
kg 310,62
(kg)
Waste, scrap steel, to disposal (kg) kg 9,67
Benefits and loads beyond the system
Unit Value
boundaries (D)
Substitution of steel (kg) kg 9,50
Substitution of stone materials (kg) kg 660,08
6 / 12
LCA: Results
The LCA results are presented below for the declared unit defined on page 2 of the EPD document.
Environmental impact
Indicator Unit A1 A2 A3 A4 A5 C1 C2 C3 C4 D
GWP-total
kg CO2 -
1,62E+02 3,90E+00 1,40E+00 7,41E+00 3,08E+00 7,08E+00 7,41E+00 4,75E-01 1,37E+00 -1,20E+01
eq
GWP-fossil
kg CO2 -
1,61E+02 3,90E+00 1,39E+00 7,40E+00 3,08E+00 7,08E+00 7,40E+00 4,69E-01 1,37E+00 -1,20E+01
eq
GWP-biogenic
kg CO2 -
8,16E-02 1,66E-03 1,27E-02 3,17E-03 5,76E-04 1,33E-03 3,17E-03 4,05E-03 1,17E-03 -3,59E-02
eq
GWP-luluc
kg CO2 -
4,86E-01 1,21E-03 1,81E-03 2,26E-03 2,42E-04 5,58E-04 2,26E-03 6,49E-04 2,69E-04 -5,70E-03
eq
kg
ODP CFC11 - 4,91E-06 9,37E-07 2,38E-07 1,79E-06 6,64E-07 1,53E-06 1,79E-06 9,24E-08 6,68E-07 -6,07E-07
eq
mol H+
AP 5,17E-01 1,43E-02 1,28E-02 2,38E-02 3,22E-02 7,40E-02 2,38E-02 3,79E-03 1,34E-02 -6,55E-02
-eq
EP-FreshWater kg P -eq 7,72E-03 3,08E-05 3,45E-05 5,89E-05 1,12E-05 2,58E-05 5,89E-05 2,96E-05 1,02E-05 -6,83E-04
EP-Marine kg N -eq 9,42E-02 3,20E-03 4,50E-03 5,22E-03 1,42E-02 3,27E-02 5,22E-03 1,11E-03 5,02E-03 -1,55E-02
mol N -
EP-Terrestial 1,34E+00 3,57E-02 5,01E-02 5,82E-02 1,56E-01 3,56E-01 5,82E-02 1,28E-02 5,53E-02 -1,65E-01
eq
kg
POCP NMVOC 5,07E-01 1,33E-02 1,38E-02 2,29E-02 4,28E-02 9,86E-02 2,29E-02 3,43E-03 1,58E-02 -6,70E-02
-eq
ADP- kg Sb-
1,49E-03 6,88E-05 3,43E-05 1,32E-04 4,72E-06 1,09E-05 1,32E-04 5,95E-06 1,21E-05 -3,15E-04
minerals&metals1 eq
ADP-fossil1 MJ 1,79E+03 6,31E+01 1,92E+01 1,20E+02 4,23E+01 9,74E+01 1,20E+02 1,46E+01 4,43E+01 -1,14E+02
WDP1 m3 2,79E+03 4,79E+01 9,72E+02 9,22E+01 8,99E+00 2,07E+01 9,22E+01 1,61E+03 9,32E+01 -6,57E+02
GWP-total = Global Warming Potential total; GWP-fossil = Global Warming Potential fossil fuels; GWP-biogenic = Global Warming Potential biogenic; GWP-luluc =
Global Warming Potential land use and land use change; ODP = Depletion potential of the stratospheric ozone layer; AP = Acidification potential, Accumulated
Exceedance; EP-freshwater = Eutrophication potential, fraction of nutrients reaching freshwater end compartment: EP-marine = Eutrophication potential, fraction of
nutrients reaching marine end compartment; EP-terrestrial = Eutrophication potential, Accumulated Exceedance; POCP = Formation potential of tropospheric ozone;
ADP-minerals&metals = Abiotic depletion potential for non-fossil resources; ADP-fossil = Abiotic depletion for fossil resources potential; WDP = Water (user)
deprivation potential, deprivation-weighted water consumption
"Reading example: 9,0 E-03 = 9,0*10-3 = 0,009"
*INA Indicator Not Assessed
1. The results of this environmental impact indicator shall be used with care as the uncertainties on these results are high or as there is limited experienced with the
indicator
Remarks to environmental impacts
7 / 12
Additional environmental impact indicators
Indicator Unit A1 A2 A3 A4 A5 C1 C2 C3 C4 D
PM Disease incidence 7,84E-06 3,54E-07 2,71E-07 6,80E-07 8,51E-07 5,92E-06 6,80E-07 6,07E-08 2,85E-07 -1,16E-06
IRP2 kgBq U235 -eq 3,75E+03 2,76E-01 1,59E-01 5,26E-01 1,81E-01 4,21E-01 5,26E-01 2,44E-01 1,92E-01 -1,97E-01
ETP-fw1 CTUe 2,52E+03 4,60E+01 3,32E+01 8,79E+01 2,31E+01 5,32E+01 8,79E+01 1,03E+01 2,19E+01 -6,09E+02
HTP-c1 CTUh 6,13E-07 0,00E+00 1,55E-09 0,00E+00 8,98E-10 1,90E-09 0,00E+00 6,60E-10 6,40E-10 -5,16E-08
HTP-nc1 CTUh 4,65E-06 4,46E-08 3,65E-08 8,50E-08 2,13E-08 4,93E-08 8,50E-08 9,24E-09 1,28E-08 1,06E-06
SQP1 dimensionless 3,56E+02 7,15E+01 5,34E+00 1,38E+02 5,37E+00 1,21E+01 1,38E+02 8,23E+00 1,61E+02 5,15E+01
PM = Particulate Matter emissions; IRP = Ionizing radiation – human health; ETP-fw = Eco toxicity – freshwater; HTP-c = Human toxicity – cancer effects; HTP-nc =
Human toxicity – non cancer effects; SQP = Potential Soil Quality Index (dimensionless)
"Reading example: 9,0 E-03 = 9,0*10-3 = 0,009"
*INA Indicator Not Assessed
1. The results of this environmental impact indicator shall be used with care as the uncertainties on these results are high or as there is limited experienced with the
indicator
2. This impact category deals mainly with the eventual impact of low dose ionizing radiation on human health of the nuclear fuel cycle. It does not consider effects due
to possible nuclear accidents, occupational exposure nor due to radioactive waste disposal in underground facilities. Potential ionizing radiation from the soil, from
radon and from some construction materials is also not measured by this indicator.
8 / 12
Resource use
Indicator Unit A1 A2 A3 A4 A5 C1 C2 C3 C4 D
PERE MJ 2,47E+02 7,89E-01 7,17E+01 1,51E+00 2,29E-01 5,29E-01 1,51E+00 7,49E+00 6,81E-01 -1,31E+01
PERM MJ 2,81E-01 0,00E+00 0,00E+00 0,00E+00 0,00E+00 0,00E+00 0,00E+00 0,00E+00 0,00E+00 0,00E+00
PERT MJ 2,48E+02 7,89E-01 7,17E+01 1,51E+00 2,29E-01 5,29E-01 1,51E+00 7,49E+00 6,81E-01 -1,31E+01
PENRE MJ 1,44E+03 6,31E+01 1,92E+01 1,20E+02 4,23E+01 9,74E+01 1,20E+02 1,46E+01 4,43E+01 -1,15E+02
PENRM MJ 4,07E+02 0,00E+00 0,00E+00 0,00E+00 0,00E+00 0,00E+00 0,00E+00 0,00E+00 0,00E+00 0,00E+00
PENRT MJ 1,85E+03 6,31E+01 1,92E+01 1,20E+02 4,23E+01 9,74E+01 1,20E+02 1,46E+01 4,43E+01 -1,15E+02
SM kg 8,30E+01 0,00E+00 0,00E+00 0,00E+00 0,00E+00 0,00E+00 0,00E+00 0,00E+00 0,00E+00 0,00E+00
RSF MJ 5,86E+01 2,75E-02 6,16E-02 5,29E-02 5,63E-03 5,63E-03 5,29E-02 0,00E+00 1,41E-02 2,55E-01
NRSF MJ 1,41E+02 9,19E-02 1,70E-01 1,77E-01 8,29E-02 8,29E-02 1,77E-01 0,00E+00 4,05E-02 1,09E+01
FW m3 1,22E+00 7,13E-03 5,83E-01 1,37E-02 2,18E-03 5,01E-03 1,37E-02 2,49E-02 5,27E-02 -9,61E-01
PERE = Use of renewable primary energy excluding renewable primary energy resources used as raw materials; PERM = Use of renewable primary energy resources used
as raw materials; PERT = Total use of renewable primary energy resources; PENRE = Use of non renewable primary energy excluding non-renewable primary energy
resources used as raw materials; PENRM = Use of non renewable primary energy resources used as raw materials; PENRT = Total use of non renewable primary energy
resources; SM = Use of secondary materials; RSF = Use of renewable secondary fuels; NRSF = Use of non-renewable secondary fuels; FW = Net use of fresh water
"Reading example: 9,0 E-03 = 9,0*10-3 = 0,009"
*INA Indicator Not Assessed
9 / 12
End of life - Waste
Indicator Unit A1 A2 A3 A4 A5 C1 C2 C3 C4 D
HWD kg 2,91E-01 3,44E-03 1,24E-02 6,58E-03 1,25E-03 2,87E-03 6,58E-03 1,45E-03 0,00E+00 -6,05E-02
NHWD kg 3,98E+02 5,42E+00 6,38E+00 1,05E+01 5,01E-02 1,15E-01 1,05E+01 4,59E-02 3,20E+02 -4,46E+00
RWD kg 1,93E-02 4,31E-04 1,35E-04 8,21E-04 2,94E-04 6,76E-04 8,21E-04 1,54E-04 0,00E+00 -1,74E-04
HWD = Hazardous waste disposed; NHWD = Non-hazardous waste disposed; RWD = Radioactive waste disposed
"Reading example: 9,0 E-03 = 9,0*10-3 = 0,009"
*INA Indicator Not Assessed
End of life - Output flow
Indicator Unit A1 A2 A3 A4 A5 C1 C2 C3 C4 D
CRU kg 2,62E-03 0,00E+00 0,00E+00 0,00E+00 0,00E+00 0,00E+00 0,00E+00 0,00E+00 0,00E+00 0,00E+00
MFR kg 0,00E+00 0,00E+00 5,98E+00 0,00E+00 0,00E+00 0,00E+00 0,00E+00 6,80E+02 0,00E+00 0,00E+00
MER kg 0,00E+00 0,00E+00 1,05E-02 0,00E+00 0,00E+00 0,00E+00 0,00E+00 0,00E+00 0,00E+00 0,00E+00
EEE MJ 0,00E+00 0,00E+00 5,68E-03 0,00E+00 0,00E+00 0,00E+00 0,00E+00 0,00E+00 0,00E+00 0,00E+00
EET MJ 0,00E+00 0,00E+00 8,59E-02 0,00E+00 0,00E+00 0,00E+00 0,00E+00 0,00E+00 0,00E+00 0,00E+00
CRU = Components for re-use; MFR = Materials for recycling; MER = Materials for energy recovery; EEE = Exported energy electrical; EET = Exported energy thermal
"Reading example: 9,0 E-03 = 9,0*10-3 = 0,009"
*INA Indicator Not Assessed
Biogenic Carbon Content
Indicator Unit At the factory gate
Biogenic carbon content in product kg C 0,00E+00
Biogenic carbon content in accompanying packaging kg C 7,68E-03
Note: 1 kg biogenic carbon is equivalent to 44/12 kg CO2
10 / 12
Additional requirements
Greenhouse gas emissions from the use of electricity in the manufacturing phase
National production mix from import, low voltage (production of transmission lines, in addition to direct emissions and losses in grid) of applied
electricity for the manufacturing process (A3).
Electricity mix Data source Amount Unit
Elektrisitet, Norge (kWh) ecoinvent 3.6 24,33 g CO2-eq/kWh
Dangerous substances
The product contains no substances given by the REACH Candidate list.
Indoor environment
The product has a very small or no impact on the indoor climate
Additional Environmental Information
Additional environmental impact indicators required in NPCR Part A for construction products
Indicator Unit A1 A2 A3 A4 A5 C1 C2 C3 C4 D
GWPIOBC kg CO2 -eq 1,62E+02 3,90E+00 1,40E+00 7,41E+00 3,08E+00 7,08E+00 7,41E+00 4,69E-01 1,37E+00 -1,73E+01
GWP-IOBC: Global warming potential calculated according to the principle of instantaneous oxidation. In order to increase the transparency of biogenic carbon​
contribution to climate impact, the indicator GWP-IOBC is required as it declares climate impacts calculated according to the principle of instantaneous oxidation.​
GWP-IOBC is also referred to as GWP-GHG in context to Swedish public procurement legislation.
11 / 12
Bibliography
ISO 14025:2010 Environmental labels and declarations - Type III environmental declarations - Principles and procedures.
ISO 14044:2006 Environmental management - Life cycle assessment - Requirements and guidelines.
EN 15804:2012+A2:2019 Environmental product declaration - Core rules for the product category of construction products.
ISO 21930:2017 Sustainability in buildings and civil engineering works - Core rules for environmental product declarations of construction
products.
ecoinvent v3, Allocation, cut-off by classification, Swiss Centre of Life Cycle Inventories.
Iversen et al., (2021) eEPD v2021.09 Background information for EPD generator tool system verification, LCA.no Report number: 07.21
Vold et al., (2022) EPD generator for concrete and concrete elements
Background information for EPD generator application and LCA data, LCA.no report number: 06.22
NPCR Part A: Construction products and services. Ver. 2.0. April 2021, EPD-Norge.
NPCR 020 Part B for concrete and concrete elements, Ver. 3.0, 20.09.2021, EPD Norway.
Program operator and publisher Phone: +47 977 22 020
The Norwegian EPD Foundation e-mail: post@epd-norge.no
Post Box 5250 Majorstuen, 0303 Oslo, Norway web: www.epd-norge.no
Owner of the declaration: Phone: +46 0522 636333
Heidelberg Materials Precast Contiga AB – Concrete e-mail: Havard.Nyman@contiga.se
Kasenabbevägen 11A,, 1662 451 91 Uddevalla, Sverige web: www.contiga.se
Author of the Life Cycle Assessment Phone: +47 916 50 916
LCA.no AS e-mail: post@lca.no
Dokka 6B, 1671 web: www.lca.no
Developer of EPD generator Phone: +47 916 50 916
LCA.no AS e-mail: post@lca.no
Dokka 6B,1671 Kråkerøy web: www.lca.no
ECO Platform web: www.eco-platform.org
ECO Portal web: ECO Portal
12 / 12
