Environmental Product Declaration
In accordance with ISO14025:2006 and EN15804:2012+A2:2019
Mono-crystalline Single glass, P-Type, solar photovoltaic modules
Owner of the declaration: Program holder and publisher:
Phono Solar Technology Co.,Ltd The Norwegian EPD foundation
Product name: Declaration number:
Mono-crystalline Single glass, P-Type, solar
photovoltaic modules
NEPD-5712-4981-EN
Registration number:
Declared unit:
1m² of manufactured photovoltaic module
NEPD-5712-4981-EN
Issue date:
Product category /PCR:
NPCR 029 2020 Part B for PV modules 1.1 Valid to: 22.12.2023
22.12.2028
The Norwegian
EPD Foundation
General information
Product:
Owner of the declaration:
Mono-crystalline Single glass, P-Type, solar
Phono Solar Technology Co.,Ltd
photovoltaic modules
Contact person: Wencong Yang
Phone: +86 25 5863 8438
Program operator:
e-mail: yangwencong@sumec.com.cn
The Norwegian EPD Foundation
Post Box 5250 Majorstuen, 0303 Oslo, Norway
Manufacturer:
Tlf: +47 23 08 80 00
Phono Solar Technology Co.,Ltd
e-mail: post@epd-norge.no
No. 1 Xinghuo Rd., Nanjing Hi-tech Zone, Nanjing,
China
Declaration number:
Phone: +86 25 5863 8438
e-mail: yangwencong@sumec.com.cn
NEPD-5712-4981-EN
This declaration is based on Product
Place of production:
Category Rules:
China
NPCR 029 2020 Part B for PV modules 1.1
Management system:
Statement of liability:
ISO 14001, ISO 9001, IEC 62941,
The owner of the declaration shall be liable for the OHSAS 18001:2007, ISO 45001
underlying information and evidence. EPD
Norway shall not be liable with respect to Organisation no:
manufacturer, life cycle assessment data and
91320191674909042W
evidences.
Issue date:
Declared unit:
1m² of manufactured photovoltaic module
22.12.2023
Valid to:
Functional unit:
1 Wp of manufactured photovoltaic module, from
cradle-to-grave and module D, with activities needed
22.12.2028
Year of study:
for a study period for a defined reference service life
(≥80% of the labelled power output) 2023
Verification:
Comparability:
Independent verification of the declaration and
EPD of construction products may not be able to
data, according to ISO14025:2010
compare if they do not comply with EN 15804 and
internal external are seen in a building context.
Sign
The EPD has been worked out by:
Laurène MEJEAN - Kapstan
[name]
Independent verifier approved by EPD Norway
Approved Manager of EPD Norway
EPD for the best environmental decision 2
Product
Product description:
Mono-crystalline solar photovoltaic modules are designed to be installed on roofs or as stand-
alone systems for local power production. All the modules included in this EPD are single glass
and the solar cells are produced with PERC process. Solar cells are assembled with the EVA, glass,
frame and electrical connections to produce the finished solar module in the production factory
in Nanjing in China.
This EPD represents multiples modules with small variations over the size, the number of cells,
power… (see table of module characteristics in “Technical details”). The results are calculated
based on the maximum inventory amongst the modules. The variation between each module
results is lower than 10 %.
Product specification:
The packaging consists of LDPE, PP, paper and a cardboard box, and the panels are delivered on
a wooden pallet.
Materials KG/DU %
Cells 3.5E-01 3%
Glass 8.1E+00 74%
EVA 9.1E-01 8%
Backsheet 5.9E+00 5%
Aluminium frame 1.1E+00 10%
Junction box 1.1E-01 0%
String connector 3.0E-02 0%
Cell connector 6.3E-02 1%
Silicone 1.6E-01 1%
Soldering flux 9.9E-03 0%
Packaging KG/DU %
Wooden pallet 5.1E-01 5%
Cardboard 1.4E-01 1%
Low density PE 1.4E-02 0%
PP 1.7E-02 0%
Plastics 9.4E-05 0%
Plastic film 6.8E-03 0%
Paper 6.7E-05 0%
Polyester film 4.2E-03 0%
EPD for the best environmental decision 3
Technical data:
This EPD is valid for the following module types:
▪ PSXXXM4-20/UH
▪ PSXXXM4-22/WH
▪ PSXXXM4-24/TH
▪ PSXXXM6-20/UH
▪ PSXXXM6-22/WH
▪ PSXXXM6(H)-24/TH
▪ PSXXXM6(H)-22/WH
▪ PSXXXM6(H)-20/UH
▪ PSXXXM6(H)-18/VH
This study has been conducted according to the requirements of:
- ISO 14044;
- ISO 14025;
- EN15804+A2:2019;
- NPCR part A “Construction products and services” version 2.0;
- NPCR part B “for photovoltaic modules used in the building and construction industry,
including production of cell, wafer, ingot block, solar grade silicon, solar substrates, solar
superstrates and other solar grade semiconductor materials” version 1.1.
Market:
World
Reference service life, product:
25 years
Additional technical information
EPD for the best environmental decision 4
Declared unit:
1m² of manufactured photovoltaic module
Cut-off criteria:
All major raw materials and all essential energy is included. The production process for raw
materials and energy flows with very small amounts (<1%) are not included. This cut-off rule
does not apply for hazardous materials and substances.
Allocation:
The allocation is made in accordance with the provisions of ISO 14025. Incoming energy and
water and waste production in-house is allocated equally among all products through mass
allocation. Effects of primary production of recycled materials allocated to the main product in
which the material was used. The recycling process and transportation of the material is allocated
to this analysis.
Data quality:
Specific data comes from actual consumption of the module assembly factory (August 2021 – July
2022). This data has been collected by the manufacturer and checked by the LCA practitioner.
Generic data is from Ecoinvent v3.6 and SimaPro v9. Characterization factors from
EN15804:2012 + A2: 2019. Generic data <10 years old.
System boundaries (X=included, MND=module not declared, MNR=module not relevant)
Benefits &
Assembly loads beyond
Product stage Use stage End of life stage
stage system
boundary
EPD for the best environmental decision 5
slairetam
waR
tropsnarT
gnirutcafunaM
tropsnarT ylbmessA
esU
ecnanetniaM
riapeR
tnemecalpeR tnemhsibrufeR
esu
ygrene
lanoitarepO
esu
retaw
lanoitarepO
noitilomed
noitcurtsnoc-eD
tropsnarT
gnissecorp
etsaW
lasopsiD
-gnilcyceR-yrevoceR-esueR
laitnetop
LCA: Calculation rules
A1 A2 A3 A4 A5 B1 B2 B3 B4 B5 B6 B7 C1 C2 C3 C4 D
X X X X MND MND MND MND MND MND MND MND X X X X X
System boundary:
The study is based on a cradle to grave analysis i.e., from raw material extraction to the disposal
of waste. A summary of what is included and excluded is shown below:
The PolySi, ingots, wafers, cells and modules are manufactured in China. The supply chain is
shown below:
Production Site
Virgin Polysi China
Ingot/brick China
Wafer China
Recycled Polysi China
Cells China
Modules China
EPD for the best environmental decision 6
LCA: Scenarios and additional technical information
The following information describe the scenarios in the different modules of the EPD.
Transport from production place to assembly/user (A4)
Transport from production place Capacity utilisation Distance Fuel/Energy
Unit Value
to assembly/user (A4) (incl. return) % (km) consumption
Truck 50% 400 Diesel (4.44E-2 L/tkm) tkm 4.65
Railway 50% 19000 Heavy fuel (2.63E-3 L/tkm) tkm 220.91
Truck 50% 1000 Diesel (4.44E-2 L/tkm) tkm 11.63
The transport step A4 covers the transport from the factories in China to the installation site in
Europe by sea and road.
Assembly (A5)
Unit Value
Kg 5.06E-01
Wooden pallet
Kg
1.37E-01
Cardboard
Kg
1.40E-02
Low density PE
Kg
1.74E-02
PP
Kg
9.41E-05
Plastics
Kg
6.83E-03
Plastic film
Kg 6.68E-05
Paper
Polyester film Kg 4.22E-03
Transportation in lorry (Capacity utilisation incl. return: 50%) Tkm 6.85E-01
The modules are installed by hand. The screwdriver electricity consumption is neglected. As in
PCR part B, the fasteners (screws) are not included in the LCA. The only impact is the packaging
waste given in the table below:
Use (B1)
The modules are considered as self-cleaning materials. No maintenance, repair, replacement, or
refurbishment is required during the module lifetime.
The modules are producing electricity from sunlight. The electricity production is calculated as
below:
𝐸 = 𝐼 ×𝑆 ×𝐸𝑓𝑓 ×𝑃𝑅×𝐷 ×(1+𝑏)
𝑦𝑒𝑎𝑟 𝑖 𝑠𝑢𝑛 1𝑘𝑊𝑝 𝑝𝑎𝑛𝑒𝑙 𝑝𝑎𝑛𝑒𝑙
Where:
- I is the sun irradiation received by the module in kWh. m-2.year-1, which depends on the
sun
site location (Norway : 1000 kWh. m-2.year-1, source : Global Solar Atlas)
- PR, or Performance Ratio, is the ratio between the energy produced by the panel and the
final energy at the output of the photovoltaic system to consider the various losses:
o The conservative PR, estimated by Global Solar Atlas, has been considered: 75%.
- Eff , or panel efficiency, is the ratio between the energy produced and the solar
panel
radiation received.
- b is the bifacial gain (5% if bifacial and 0% if monofacial)
- S is the surface area to get 1 kWp.
1kWp
EPD for the best environmental decision 7
- D corresponds to the degradation of the panel in year i. For example, in this EPD, the
panel
degradation is 2% the first year and then 55% per year. D =0.98 × (1-0.55%)i-1.
panel
Solar irradiance for electricity production Unit Value
1000 kWh/m²/year kWh/m² (25 years) 3 734
1100 kWh/m²/year kWh/m² (25 years) 4 107
1200 kWh/m²/year kWh/m² (25 years) 4 480
1300 kWh/m²/year kWh/m² (25 years) 4 854
1400 kWh/m²/year kWh/m² (25 years) 5 227
1500 kWh/m²/year kWh/m² (25 years) 5 601
1600 kWh/m²/year kWh/m² (25 years) 5 974
1700 kWh/m²/year kWh/m² (25 years) 6 347
Maintenance (B2)/Repair (B3)/ Replacement (B4)/Refurbishment (B5)
The modules are considered as self-cleaning materials. No maintenance, repair, replacement, or
refurbishment is required during the module lifetime.
Operational energy (B6) and water consumption (B7)
The products do not require any energy or water consumption.
End of Life (C1, C3, C4)
The modules are considered as removed by hand. Waste scenarios follow PCR part B standards
for C3 and C4.
Waste process Unit Value
Recycling Kg 2.38E+01
Incineration and energy recovery Kg 1.24E+00
Transport to waste processing (C2)
It has been assumed that the modules are collected by truck and sent for recycling. 50 km is
considered from the site to the recycling factory as proposed in PCR part B.
Capacity Value
Type utilisation Type of vehicle Distance (km) Fuel/Energy consumption
(incl. return) % (tkm)
Truck 50% 16-32 metric ton lorry, EURO5 50 Diesel (4.44E-2 l/tkm) 6.19E-01
Benefits and loads beyond the system boundaries (D)
Benefits and loads have been based on glass and aluminium frame recycling only. Energy
recovery from A4-A5 and C1-C4 modules is included.
Item Unit Value
Glass Kg -8.05E+00
Aluminium Kg -2.87E-01
Energy recovery EEE MJ 4.06E+01
Energy recovery ETE MJ 1.74E+01
EPD for the best environmental decision 8
LCA: Results
The LCA results show the environmental impacts and resource input and output flows calculated
according to ISO 14025 and EN 15804 +A2. The results are shown per functional unit, which for
this declaration is 1Wp, as well as per declared unit, which for this declaration is 1 m². The LCA
results have been calculated using the LCA software SimaPro 9.
Core environmental impact indicators (per functional unit - Wp)
Parameter Unit Total A1-A3 A4 A5 B1 - B7 C1 C2 C3 C4 D
GWP-total kg CO2 eq 8.38E-01 8.36E-01 2.25E-02 5.85E-03 0.00E+00 0.00E+00 2.62E-04 1.08E-03 6.06E-04 -2.80E-02
GWP-fossil kg CO2 eq 8.35E-01 8.36E-01 2.24E-02 1.54E-03 0.00E+00 0.00E+00 2.61E-04 1.07E-03 6.05E-04 -2.76E-02
GWP-
kg CO2 eq 2.76E-03 -1.29E-03 7.53E-06 4.31E-03 0.00E+00 0.00E+00 1.04E-07 3.08E-06 1.27E-06 -2.73E-04
biogenic
GWP-luluc kg CO2 eq 6.68E-04 7.44E-04 1.21E-05 2.65E-07 0.00E+00 0.00E+00 9.40E-08 5.19E-07 4.03E-07 -8.93E-05
kg CFC11
ODP 5.37E-07 5.34E-07 4.83E-09 1.31E-10 0.00E+00 0.00E+00 6.24E-11 1.38E-11 3.59E-11 -1.44E-09
eq
AP mol H+ eq 4.88E-03 4.69E-03 3.67E-04 2.81E-06 0.00E+00 0.00E+00 1.09E-06 1.34E-06 1.97E-06 -1.84E-04
EP-
kg P eq 4.15E-05 4.22E-05 1.29E-07 6.27E-09 0.00E+00 0.00E+00 1.79E-09 5.21E-09 1.37E-08 -8.95E-07
freshwater
EP-marine kg N eq 1.05E-03 9.86E-04 9.28E-05 9.05E-07 0.00E+00 0.00E+00 3.30E-07 3.65E-07 5.59E-07 -2.89E-05
EP-
mol N eq 1.06E-02 9.84E-03 1.03E-03 9.82E-06 0.00E+00 0.00E+00 3.64E-06 4.92E-06 6.43E-06 -3.19E-04
terrestial
kg
POCP NMVOC 3.76E-03 3.57E-03 2.75E-04 2.85E-06 0.00E+00 0.00E+00 1.17E-06 1.02E-06 1.66E-06 -9.34E-05
eq
ADP-M&M² kg Sb eq 4.33E-05 4.31E-05 5.75E-08 2.07E-09 0.00E+00 0.00E+00 6.00E-10 3.33E-09 1.96E-09 1.04E-07
ADP-fossil² MJ 9.64E+00 9.63E+00 3.15E-01 8.98E-03 0.00E+00 0.00E+00 4.08E-03 2.42E-03 3.72E-03 -3.15E-01
WDP² m3 4.55E-01 4.56E-01 7.74E-04 1.55E-04 0.00E+00 0.00E+00 1.36E-05 2.12E-04 7.75E-05 -2.96E-03
GWP-total: Global Warming Potential; GWP-fossil: Global Warming Potential fossil fuels; GWP-biogenic: Global Warming Potential
biogenic; GWP-LULUC: Global Warming Potential land use and land use change; ODP: Depletion potential of the stratospheric ozone
layer; AP: Acidification potential, Accumulated Exceedance; EP-freshwater: Eutrophication potential, fraction of nutrients reaching
freshwater end compartment; See “additional Norwegian requirements” for indicator given as PO4 eq. EP-marine: Eutrophication
potential, fraction of nutrients reaching freshwater end compartment; EP-terrestrial: Eutrophication potential, Accumulated
Exceedance; POCP: Formation potential of tropospheric ozone; ADP-M&M: Abiotic depletion potential for non-fossil resources
(minerals and metals); ADP-fossil: Abiotic depletion potential for fossil resources; WDP: Water deprivation potential, deprivation
weighted water counsumption
Reading example: 9,0 E-03 = 9,0*10-3 = 0,009
Additional environmental impact indicators (per functional unit - Wp)
Parameter Unit Total A1-A3 A4 A5 B1 - B7 C1 C2 C3 C4 D
Disease
PM 5.58E-08 5.67E-08 1.17E-09 4.16E-11 0.00E+00 0.00E+00 2.35E-11 1.29E-11 1.72E-11 -2.17E-09
incidence
kBq U235
IRP 2.06E-02 1.97E-02 1.35E-03 3.91E-05 0.00E+00 0.00E+00 1.77E-05 3.07E-05 1.28E-05 -4.57E-04
eq.
ETP-fw CTUe 2.79E+01 2.83E+01 2.30E-01 1.14E-02 0.00E+00 0.00E+00 3.18E-03 7.59E-03 4.81E-02 -7.28E-01
HTP-c CTUh 7.43E-10 7.39E-10 1.07E-11 4.87E-13 0.00E+00 0.00E+00 8.81E-14 4.81E-13 2.59E-11 -3.37E-11
HTP-nc CTUh 3.18E-08 3.20E-08 2.07E-10 1.70E-11 0.00E+00 0.00E+00 3.48E-12 1.25E-11 1.39E-10 -5.96E-10
Dimensio
SQP 2.81E+01 2.81E+01 2.00E-01 8.68E-03 0.00E+00 0.00E+00 7.18E-03 4.94E-03 7.79E-03 -1.86E-01
nless
PM: Particulate matter emissions; IRP: Ionising radiation, human health; ETP-fw: Ecotoxicity (freshwater); ETP-c: Human toxicity,
cancer effects; HTP-nc: Human toxicity, non-cancer effects; SQP: Land use related impacts / soil quality
EPD for the best environmental decision 9
1 This impact category deals mainly with the eventual impact of low dose ionizing radiation on human health of the nuclear fuel
cycle. It does not consider effects due to possible nuclear accidents, occupational exposure nor due to radioactive waste disposal
in underground facilities. Potential ionizing radiation from the soil, from radon and from some construction materials is also not
measured by this indicator.
2 The results of this environmental impact indicator shall be used with care as the uncertainties on these results are high or as
there is limited experienced with the indicator
Resource use (per functional unit - Wp)
Parameter Unit Total A1-A3 A4 A5 B1 - B7 C1 C2 C3 C4 D
RPEE MJ 2.34E+00 2.35E+00 3.39E-03 1.91E-04 0.00E+00 0.00E+00 5.19E-05 1.30E-02 1.79E-04 -3.18E-02
RPEM MJ 0.00E+00 0.00E+00 0.00E+00 0.00E+00 0.00E+00 0.00E+00 0.00E+00 0.00E+00 0.00E+00 0.00E+00
TPE MJ 2.34E+00 2.35E+00 3.39E-03 1.91E-04 0.00E+00 0.00E+00 5.19E-05 1.30E-02 1.79E-04 -3.18E-02
NRPE MJ 9.64E+00 9.62E+00 3.15E-01 8.97E-03 0.00E+00 0.00E+00 4.08E-03 2.38E-03 3.72E-03 -3.15E-01
NRPM MJ 0.00E+00 0.00E+00 0.00E+00 0.00E+00 0.00E+00 0.00E+00 0.00E+00 0.00E+00 0.00E+00 0.00E+00
TRPE MJ 9.63E+00 9.61E+00 3.15E-01 8.97E-03 0.00E+00 0.00E+00 4.07E-03 2.38E-03 3.72E-03 -3.15E-01
SM kg 0.00E+00 0.00E+00 0.00E+00 0.00E+00 0.00E+00 0.00E+00 0.00E+00 0.00E+00 0.00E+00 0.00E+00
RSF MJ 0.00E+00 0.00E+00 0.00E+00 0.00E+00 0.00E+00 0.00E+00 0.00E+00 0.00E+00 0.00E+00 0.00E+00
NRSF MJ 0.00E+00 0.00E+00 0.00E+00 0.00E+00 0.00E+00 0.00E+00 0.00E+00 0.00E+00 0.00E+00 0.00E+00
W m3 1.16E-02 1.15E-02 2.45E-05 3.26E-06 0.00E+00 0.00E+00 4.39E-07 9.67E-05 1.98E-06 -6.72E-05
RPEE Renewable primary energy resources used as energy carrier; RPEM Renewable primary energy resources used as raw materials;
TPE Total use of renewable primary energy resources; NRPE Nonrenewable primary energy resources used as energy carrier; NRPM
Nonrenewable primary energy resources used as materials; TRPE Total use of non-renewable primary energy resources; SM Use of
secondary materials; RSF Use of renewable secondary fuels; NRSF Use of non-renewable secondary fuels; W Use of net fresh water.
End of life – Waste (per functional unit - Wp)
Parameter Unit Total A1-A3 A4 A5 B1 - B7 C1 C2 C3 C4 D
HW KG 8.03E-02 7.98E-02 2.74E-04 5.16E-04 0.00E+00 0.00E+00 2.82E-06 4.95E-04 3.65E-03 -4.39E-03
NHW KG 7.85E-01 7.92E-01 1.18E-02 4.92E-04 0.00E+00 0.00E+00 4.02E-04 2.28E-04 1.61E-04 -1.98E-02
RW KG 2.02E-05 1.85E-05 2.14E-06 5.85E-08 0.00E+00 0.00E+00 2.76E-08 1.68E-08 1.75E-08 -5.23E-07
HW Hazardous waste disposed; NHW Non-hazardous waste disposed; RW Radioactive waste disposed.
End of life – output flow (per functional unit - Wp)
Parameter Unit Total A1-A3 A4 A5 B1 - B7 C1 C2 C3 C4 D
CR kg 0.00E+00 0.00E+00 0.00E+00 0.00E+00 0.00E+00 0.00E+00 0.00E+00 0.00E+00 0.00E+00 0.00E+00
MR kg 1.12E-01 0.00E+00 0.00E+00 0.00E+00 0.00E+00 0.00E+00 0.00E+00 1.11E-01 0.00E+00 0.00E+00
MER kg 0.00E+00 0.00E+00 0.00E+00 0.00E+00 0.00E+00 0.00E+00 0.00E+00 0.00E+00 0.00E+00 0.00E+00
EEE MJ 3.19E-01 0.00E+00 0.00E+00 0.00E+00 0.00E+00 0.00E+00 0.00E+00 1.31E-01 0.00E+00 1.88E-01
ETE MJ 5.62E-02 0.00E+00 0.00E+00 0.00E+00 0.00E+00 0.00E+00 0.00E+00 5.62E-02 0.00E+00 0.00E+00
Exported
energy - gas MJ 8.05E-02 0.00E+00 0.00E+00 0.00E+00 0.00E+00 0.00E+00 0.00E+00 0.00E+00 0.00E+00 8.05E-02
and process
CR Components for reuse; MR Materials for recycling; MER Materials for energy recovery; EEE Exported electric energy; ETE Exported
thermal energy.
EPD for the best environmental decision 10
Information describing the biogenic carbon content at the factory gate (per
functional unit - Wp)
Biogenic carbon content Unit Value
Biogenic carbon content in product kg C 0.00E+00
Biogenic carbon content in the accompanying packaging kg C 1.18E-03
Results presented per declared unit
Core environmental impact indicators (per declared unit - m2)
Parameter Unit Total A1-A3 A4 A5 B1 - B7 C1 C2 C3 C4 D
GWP-total kg CO2 eq 1.80E+02 1.80E+02 4.82E+00 1.26E+00 0.00E+00 0.00E+00 5.62E-02 2.31E-01 1.30E-01 -6.02E+00
GWP-fossil kg CO2 eq 1.79E+02 1.80E+02 4.82E+00 3.31E-01 0.00E+00 0.00E+00 5.62E-02 2.31E-01 1.30E-01 -5.94E+00
GWP-
kg CO2 eq 5.93E-01 -2.78E-01 1.62E-03 9.27E-01 0.00E+00 0.00E+00 2.24E-05 6.62E-04 2.74E-04 -5.87E-02
biogenic
GWP-
kg CO2 eq 1.44E-01 1.60E-01 2.61E-03 5.69E-05 0.00E+00 0.00E+00 2.02E-05 1.11E-04 8.65E-05 -1.92E-02
LULUC
kg CFC11
ODP 1.15E-04 1.15E-04 1.04E-06 2.82E-08 0.00E+00 0.00E+00 1.34E-08 2.96E-09 7.72E-09 -3.10E-07
eq
AP mol H+ eq 1.05E+00 1.01E+00 7.88E-02 6.05E-04 0.00E+00 0.00E+00 2.34E-04 2.87E-04 4.23E-04 -3.95E-02
EP-
kg P eq 8.91E-03 9.07E-03 2.78E-05 1.35E-06 0.00E+00 0.00E+00 3.84E-07 1.12E-06 2.95E-06 -1.92E-04
freshwater
EP-marine kg N eq 2.26E-01 2.12E-01 1.99E-02 1.95E-04 0.00E+00 0.00E+00 7.08E-05 7.84E-05 1.20E-04 -6.20E-03
EP-
mol N eq 2.27E+00 2.11E+00 2.21E-01 2.11E-03 0.00E+00 0.00E+00 7.82E-04 1.06E-03 1.38E-03 -6.86E-02
terrestial
kg
POCP NMVOC 8.08E-01 7.67E-01 5.90E-02 6.12E-04 0.00E+00 0.00E+00 2.52E-04 2.19E-04 3.56E-04 -2.01E-02
eq
ADP-M&M kg Sb eq 9.29E-03 9.26E-03 1.23E-05 4.45E-07 0.00E+00 0.00E+00 1.29E-07 7.14E-07 4.21E-07 2.23E-05
ADP-fossil MJ 2.07E+03 2.07E+03 6.77E+01 1.93E+00 0.00E+00 0.00E+00 8.76E-01 5.20E-01 7.99E-01 -6.76E+01
m3
WDP 9.77E+01 9.80E+01 1.66E-01 3.33E-02 0.00E+00 0.00E+00 2.93E-03 4.55E-02 1.66E-02 -6.35E-01
depriv.
GWP-total: Global Warming Potential; GWP-fossil: Global Warming Potential fossil fuels; GWP-biogenic:
Global Warming Potential biogenic; GWP-LULUC: Global Warming Potential land use and land use change;
ODP: Depletion potential of the stratospheric ozone layer; AP: Acidification potential, Accumulated
Exceedance; EP-freshwater: Eutrophication potential, fraction of nutrients reaching freshwater end
compartment; See “additional Norwegian requirements” for indicator given as PO4 eq. EP-marine:
Eutrophication potential, fraction of nutrients reaching freshwater end compartment; EP-terrestial:
Eutrophication potential, Accumulated Exceedance; POCP: Formation potential of tropospheric ozone; ADP-
M&M: Abiotic depletion potential for non-fossil resources (minerals and metals); ADP-fossil: Abiotic
depletion potential for fossil resources; WDP: Water deprivation potential, deprivation weighted water
counsumption
Additional environmental impact indicators (per declared unit - m2)
Parameter Unit Total A1-A3 A4 A5 B1 - B7 C1 C2 C3 C4 D
Disease
PM 1.20E-05 1.22E-05 2.52E-07 8.94E-09 0.00E+00 0.00E+00 5.06E-09 2.77E-09 3.69E-09 -4.66E-07
incidence
kBq U235
IRP 4.44E+00 4.22E+00 2.90E-01 8.41E-03 0.00E+00 0.00E+00 3.80E-03 6.61E-03 2.75E-03 -9.81E-02
eq.
ETP-fw CTUe 5.99E+03 6.08E+03 4.95E+01 2.45E+00 0.00E+00 0.00E+00 6.84E-01 1.63E+00 1.03E+01 -1.56E+02
EPD for the best environmental decision 11
HTP-c CTUh 1.60E-07 1.59E-07 2.29E-09 1.05E-10 0.00E+00 0.00E+00 1.89E-11 1.03E-10 5.56E-09 -7.23E-09
HTP-nc CTUh 6.82E-06 6.87E-06 4.44E-08 3.66E-09 0.00E+00 0.00E+00 7.48E-10 2.69E-09 3.00E-08 -1.28E-07
Dimensio
SQP 6.04E+03 6.03E+03 4.29E+01 1.86E+00 0.00E+00 0.00E+00 1.54E+00 1.06E+00 1.67E+00 -3.99E+01
nless
PM: Particulate matter emissions; IRP: Ionising radiation, human health; ETP-fw: Ecotoxicity (freshwater);
ETP-c: Human toxicity, cancer effects; HTP-nc: Human toxicity, non-cancer effects; SQP: Land use related
impacts / soil quality
Resource use (per declared unit - m2)
Parameter Unit Total A1-A3 A4 A5 B1 - B7 C1 C2 C3 C4 D
RPEE MJ 5.02E+02 5.05E+02 7.29E-01 4.10E-02 0.00E+00 0.00E+00 1.11E-02 2.80E+00 3.84E-02 -6.84E+00
RPEM MJ 0.00E+00 0.00E+00 0.00E+00 0.00E+00 0.00E+00 0.00E+00 0.00E+00 0.00E+00 0.00E+00 0.00E+00
TPE MJ 5.02E+02 5.05E+02 7.29E-01 4.10E-02 0.00E+00 0.00E+00 1.11E-02 2.80E+00 3.84E-02 -6.84E+00
NRPE MJ 2.07E+03 2.07E+03 6.77E+01 1.93E+00 0.00E+00 0.00E+00 8.76E-01 5.12E-01 7.99E-01 -6.77E+01
NRPM MJ 0.00E+00 0.00E+00 0.00E+00 0.00E+00 0.00E+00 0.00E+00 0.00E+00 0.00E+00 0.00E+00 0.00E+00
TRPE MJ 2.07E+03 2.07E+03 6.77E+01 1.93E+00 0.00E+00 0.00E+00 8.75E-01 5.12E-01 7.98E-01 -6.76E+01
SM kg 0.00E+00 0.00E+00 0.00E+00 0.00E+00 0.00E+00 0.00E+00 0.00E+00 0.00E+00 0.00E+00 0.00E+00
RSF MJ 0.00E+00 0.00E+00 0.00E+00 0.00E+00 0.00E+00 0.00E+00 0.00E+00 0.00E+00 0.00E+00 0.00E+00
NRSF MJ 0.00E+00 0.00E+00 0.00E+00 0.00E+00 0.00E+00 0.00E+00 0.00E+00 0.00E+00 0.00E+00 0.00E+00
W m3 2.48E+00 2.47E+00 5.26E-03 7.00E-04 0.00E+00 0.00E+00 9.44E-05 2.08E-02 4.25E-04 -1.44E-02
RPEE Renewable primary energy resources used as energy carrier; RPEM Renewable primary energy
resources used as raw materials; TPE Total use of renewable primary energy resources; NRPE Non
renewable primary energy resources used as energy carrier; NRPM Non renewable primary energy
resources used as materials; TRPE Total use of non renewable primary energy resources; SM Use of
secondary materials; RSF Use of renewable secondary fuels; NRSF Use of non renewable secondary fuels; W
Use of net fresh water
End of life – Waste (per declared unit - m2)
Parameter Unit Total A1-A3 A4 A5 B1 - B7 C1 C2 C3 C4 D
HW KG 1.73E+01 1.71E+01 5.89E-02 1.11E-01 0.00E+00 0.00E+00 6.06E-04 1.06E-01 7.85E-01 -9.43E-01
NHW KG 1.69E+02 1.70E+02 2.54E+00 1.06E-01 0.00E+00 0.00E+00 8.64E-02 4.90E-02 3.46E-02 -4.26E+00
RW KG 4.34E-03 3.97E-03 4.60E-04 1.26E-05 0.00E+00 0.00E+00 5.93E-06 3.61E-06 3.75E-06 -1.12E-04
HW Hazardous waste disposed; NHW Non hazardous waste disposed; RW Radioactive waste disposed
EPD for the best environmental decision 12
End of life – output flow (per declared unit - m2)
Parameter Unit Total A1-A3 A4 A5 B1 - B7 C1 C2 C3 C4 D
CR kg 0.00E+00 0.00E+00 0.00E+00 0.00E+00 0.00E+00 0.00E+00 0.00E+00 0.00E+00 0.00E+00 0.00E+00
MR kg 2.41E+01 0.00E+00 0.00E+00 0.00E+00 0.00E+00 0.00E+00 0.00E+00 2.38E+01 0.00E+00 0.00E+00
MER kg 0.00E+00 0.00E+00 0.00E+00 0.00E+00 0.00E+00 0.00E+00 0.00E+00 0.00E+00 0.00E+00 0.00E+00
EEE MJ 6.85E+01 0.00E+00 0.00E+00 0.00E+00 0.00E+00 0.00E+00 0.00E+00 2.82E+01 0.00E+00 4.03E+01
ETE MJ 1.21E+01 0.00E+00 0.00E+00 0.00E+00 0.00E+00 0.00E+00 0.00E+00 1.21E+01 0.00E+00 0.00E+00
Exported
energy - gas MJ 1.73E+01 0.00E+00 0.00E+00 0.00E+00 0.00E+00 0.00E+00 0.00E+00 0.00E+00 0.00E+00 1.73E+01
and process
CR Components for reuse; MR Materials for recycling; MER Materials for energy recovery; EEE Exported
electric energy; ETE Exported thermal energy
Reading example: 9,0 E-03 = 9,0*10-3 = 0,009
Information describing the biogenic carbon content at the factory gate (per
declared unit - m2)
Biogenic carbon content Unit Value
Biogenic carbon content in product kg C 0.00E+00
Biogenic carbon content in the accompanying packaging kg C 2.53E-01
EPD for the best environmental decision 13
Additional requirements
Location based electricity mix from the use of electricity in manufacturing
National production mix from import, low voltage (production of transmission lines, in addition
to direct emissions and losses in grid) of applied electricity for the manufacturing prosess
(foreground/core) per functional unit.
National electricity grid A3 (kWh/m²) Value (kgCO2eq/kWh)
PS_Electricity, medium voltage {CN-JS} market group for Cut-off, U 4.1E+00 1.06
Guarantees of origin from the use of electricity in the manufacturing phase
In the context of China, a market-based approach is not applicable due to the absence of a
Guarantee of Origin system. Therefore, a location-based approach is employed to assess the
environmental impact of electricity in this EPD. National production mix from import, medium
voltage (production of transmission lines, in addition to direct emissions and losses in grid) of
applied electricity for the manufacturing process (A3).
Additional environmental impact indicators required for construction products (Wp)
In order to increase the transparency of biogenic carbon contribution to climate impact, the
indicator GWP-IOBC is required as it declares climate impacts calculated according to the
principle of instantanious oxidation. GWP-IOBC is also reffered to as GWP-GHG in context to
Swedish public procurement legislation.
Parameter Unit Total A1-A3 A4 A5 B1 - B7 C1 C2 C3 C4 D
GWP-IOBC KG 8.35E-01 8.36E-01 2.24E-02 1.54E-03 0.00E+00 0.00E+00 2.61E-04 1.07E-03 6.05E-04 -2.76E-02
GWP-IOBC Global warming potential calculated according to the principle of instantaneous oxidation.
Hazardous substances
The declaration is based upon reference to threshold values and/or test results and/or material
safety data sheets provided to EPD verifiers. Documentation available upon request to EPD
owner.
□ The product contains substances given by the REACH Candidate list that are less than
0,1 % by weight.
Indoor environment
No tests have been carried out on the product concerning indoor climate.
Carbon footprint (A1-C4)
The carbon footprint per kWh with a production in Norway (I =1000 kWh. m-2.year-1 ) is 48.22
rad
gCO2-eq / kWh.
The carbon footprint per kWh with a production in Italy (I =1600 kWh. m-2.year-1 ) is 32.15
rad
gCO2-eq / kWh.
EPD for the best environmental decision 14
Extrapolation rules
Power peak
The environmental impacts are given for a specific module power peak, Wp = 555Wp. For a
EPD1
different Wp (for example Wp = 460Wp), the impacts can be re-calculated by applying to
project
each impact the following ratio: Wp / Wp = 555 Wp / 460 Wp.
project EPD
Indeed, the 555 Wp and 460 Wp modules have the same impact per module (Impact ).
module
Therefore:
𝑖𝑚𝑝𝑎𝑐𝑡 𝐼𝑚𝑝𝑎𝑐𝑡 555
𝑚𝑜𝑑𝑢𝑙𝑒 𝑚𝑜𝑑𝑢𝑙𝑒
𝐼𝑚𝑝𝑎𝑐𝑡𝑠 = = ×
𝑝𝑟𝑜𝑗𝑒𝑐𝑡 (𝑝𝑒𝑟 𝑘𝑊𝑝) 460 555 460
555
= 𝐼𝑚𝑝𝑎𝑐𝑡𝑠 ×
𝐸𝑃𝐷 (𝑝𝑒𝑟 𝑘𝑊𝑝) 460
EPD for the best environmental decision 15
Bibliography
ISO 14025:2010 Environmental labels and declarations - Type III environmental
declarations - Principles and procedures
ISO 14044:2006 Environmental management - Life cycle assessment -
Requirements and guidelines
EN 15804:2012+A2:2019 Sustainability of construction works - Environmental product
declaration - Core rules for the product category of construction
products
ISO 21930:2007 Sustainability in building construction - Environmental
declaration of building products
Program Operator tlf +47 23 08 80 00
The Norwegian EPD Foundation
Post Box 5250 Majorstuen, 0303 Oslo e-post: post@epd-norge.no
Norway web www.epd-norge.no
Publisher tlf +47 23 08 80 00
The Norwegian EPD Foundation
Post Box 5250 Majorstuen, 0303 Oslo e-post: post@epd-norge.no
Norway web www.epd-norge.no
Owner of the declaration tlf +86 25 5863 8438
Phono Solar Technology Co.,Ltd Fax
1 Xing Huo Lu, Pukou District,
e-post: yangwencong@sumec.com.cn
Nanjing, Jiangsu, 211531
China web http://www.phonosolar.com/
Author of the life cycle assesment tlf +33 6 80 90 58 02
Kapstan Fax
28 rue Bellicard, 69003 Lyon e-post: Laurene.mejean@kapstan.fr
France web www.kapstan.fr
ECO Platform web www.eco-platform.org
ECO Portal web ECO Portal
EPD for the best environmental decision 16
