Environmental Product
Declaration
In accordance with ISO 14025
Hydroelectricity from Skjerka power station
Owner of the declaration: Product:
AS
Hydroelectricity from
Å Energi Vannkraft Skjerka power station
Program holder and publisher:
The Norwegian EPD foundation
Declaration number:
Manufacturer:
NEPD-3466-2067-EN
Registration Number:
Å Energi Vannkraft
NEPD-3466-2067-EN AS
Issue date:
Valid to:
03.05.2022
The Norwegian 03.05.2027
EPD Foundation
ver-100223
General information
Product:
Electricity from hydropower
Owner of the declaration:
AS
Program Holder:
Contact person: Oliver Germeroth
The Norwegian EPD Foundation Å Energi Vannkraft
Phone: +49 (0) 179 6612 758
Post Box 5250 Majorstuen, 0303 Oslo, Norway
e-mail:
Tlf: +47 23 08 80 00
e-post: post@epd-norge.no oliver.germeroth@aenergi.no
Manufacturer:
Decl ration Number:
Postboks 603 Lundsiden, 4606 Kristiansand
Å Energi Vannkraft AS
Phone: + 47 38 60 70 00
a
e-mail: firmapost@ae.no
NEPD-3466-2067-EN
This declaration is based on Product
Category Rules: Place of production:
PCR 2007:08, v.4.2 Electricity, steam and hot/cold Skjerkevatn, Åseral kommune, Norway
water generation and distribution.
Management system:
Statements:
The owner of the declaration shall be liable for the
underlying information and evidence. EPD
Organisation no:
Norway shall not be liable with respect to
882973972
manufacturer, life cycle assessment data and
evidences.
Issue date:
Declared unit:
1 kWh electricity produced and thereafter 03.05.2022
Valid to:
distributed to cosnumer.
Declared unit with option:
03.05.2027
Year of study:
1 kWh electricity produced and thereafter
2021
distributed to co sumer.
n Comparability:
Functional unit:
EPDs from other programmes than the Norwegian
EPD Foundation may not be comparable.
Verification:
Independent verification of the declaration and
The EPD has been worked out by:
data, according to ISO14025:2010
Ellen Soldal, NORSUS
internal External X
Mie Vold, LCA.no AS
(Independent verifier approved by EPD Norway) Approved (Manager of EPD Norway)
EPD for the best environmental decision 2
Product
Product description:
110 kV hydroelectricity produced at Skjerka power station and dsitributed to consumer. The
power station is located in Åseral municipality in southern parts of Norway.
Technical data:
High voltage (110 kV) hydroelectricity.
Market:
Europe
Reference service life:
NA
LCA: Calculation rules
Declated unit:
1 kWh electricity produced and distributed to consumers.
During transformation and transmission there will be loss of electricity. Loss of electricity has
been included, and the loss is based on ecoinvent 3.7.1. Due to loss in transformation and
transmission, electricity delivered to customers is 0,9 kWh.
Energy loss due to distribution
Voltage Loss in % Loss in kWh Source
High 2,7 % 0.027 kWh Wernet et al. 2016
Medium 1,1 % 0.011 kWh Wernet et al. 2016
Low 6,0 % 0.058 kWh Wernet et al. 2016
Data quality:
Information on material flows are based on site specific data. The data was collected partly in
2015 and partly in 2021. Due to long life-time of infrastructure, the data is considered to be
relevant to time, geography and technology. The production of raw materials are based on
generic data from the ecoinvent database, version 3.7.1 (Wernet et al. 2016).
Allocation:
The allocation is made in accordance with the provisions of ISO 14025. Effects of primary
production of recycled materials are allocated to the main product in wich the material was
used. The recycling process and transportation of recyled material are allocated to the user. In
line with the PCR 2007:08, v.4.2 (Environdec 2021), some of the environmental burdens related
to the infrastructuer, are allocated to downstream power station. The environmental impacts
from dams, gates and roads upstream Skjerka and at Skjerka are allocated to Skjerka power
EPD for the best environmental decision 3
station and to Håverstad power station which is downstream Skjerka power station. The
allocation is based on annual electricity generation and Skjerka power station recieves 70% of
the environmental load.
Error! Reference source not found. shows the structure of the LCA-model. It illustrates which
life cycle stages that are included and whether the data used is generic or specific.
System boundary:
The total contribution to environmental impacts for electricity generation and distribution are
included. This includes raw material extraction, production and transportation, maintenance,
operation and transmission (Figure 1). Dams include four upstream dams, which provide
benefit to the electricity generation at Skjerka power station, and dams at Skjerka power
station.
100% reinvestment of all installations are includede, divided over the technical lifetime of the
installations. The environmental impacts from dams, gates and roads upstream and at Skjerka
are allocated to Skjerka power station and Håverstad power station, which is downstream
Skjerka. The allocation is based on annual electricity generation, and Skjerka power station is
given 70% of the load.
Cut-off criteria:
All major raw materials and all essential energy is included. In this analysis, no data obtained
has been omitted. All data and processes have been considered relevant and all the data
attained has been analyzed.
EPD for the best environmental decision 4
The following information describe the scenarios in the different modules of the EPD.
A4 includes distribution of electricity generated. Distribution network from ecoinvent 3.7.1 is
used. This includes distribution network, loss in transformation and transmission, acquisition
and emissions of sulfur hexafluoride. Transformation and transmission leads to loss of
electricity, thus, delivered electricity is less than 1 kWh. No modules after A4 have been
included.
For the generation of electricity from reservoir hydro power, emissions of GHG from inundated
land is the single most important contribution to the GWP and to eutrophication (EP).
Emissions of GHG from inundated land stands for 42% of the total impact in GWP. For the other
impact categories, distribution of electricity is the most important.
System boundaries (X = included, MND = module not declared, MNR = module not relevant)
After
Assembly
Product stage Use stage End of life stage end-of-
stage
life
EPD for the best environmental decision 5
slairetam
waR
tropsnarT
gnirutcafunaM
tropsnarT ylbmessA
esU
ecnanetniaM
riapeR
tnemecalpeR tnemhsibrufeR
esu
ygrene
lanoitarepO
esu
retaw
lanoitarepO
noitilomed
noitcurtsnoc-eD
tropsnarT
gnissecorp
etsaW
lasopsiD
-gnilcyceR-yrevoceR-esueR
laitnetop
LCA: Scenarios and additional technical information
LCA: Results
A1 A2 A3 A4 A5 B1 B2 B3 B4 B5 B6 B7 C1 C2 C3 C4
X X X X MNR MNR MNR MNR MNR MNR MNR MNR MNR MNR MNR MNR MNR
Environmental impact
Parameter Unit A1-A2 A3 A4 A1-A4
GWP – Total kg CO2 -eq. 7,44E-04 1,96E-03 1,84E-03 4,54E-03
GWP – Fossil kg CO2 -eq. 7,20E-04 1,96E-03 1,80E-03 4,48E-03
GWP – Biogent kg CO2 -eq. 2,44E-05 4,82E-08 3,82E-05 6,27E-05
GWP – Land use and land
kg CO2 -eq. 3,80E-07 2,74E-09 2,43E-06 2,81E-06
use change
ODP kg CFC11-eq. 2,86E-11 1,15E-11 1,42E-10 1,82E-10
POCP kg C2H4 -eq. 1,90E-07 1,13E-08 8,99E-07 1,10E-06
AP kg SO2 -eq. 5,67E-06 3,83E-07 2,22E-05 2,83E-05
EP kg PO43--eq. 1,08E-06 6,57E-05 3,17E-06 6,99E-05
ADPM kg Sb-eq. 1,47E-08 1,14E-11 2,12E-06 2,14E-06
ADPE MJ 4,98E-03 8,95E-04 1,91E-02 2,49E-02
AWARE m3 1,10E-04 4,83E-04 1,55E-03 2,14E-03
GWP Global warming potential, divided into fossil, biogenic and land use and land use change ; ODP
Depletion potential of the stratospheric ozone layer; POCP Formation potential of tropospheric
photochemical oxidants; AP Acidification potential of land and water; EP Eutrophication potential; ADPM
Abiotic depletion potential for non fossil resources; ADPE Abiotic depletion potential for fossil resources;
AWARE Relative Available WAter Remaining.
Resource use
Parameter Unit A1-A2 A3 A4 A1-A4
RPEE MJ 3,45E+00 2,40E-06 5,64E-03 3,45E+00
RPEM MJ 0,00E+00 0,00E+00 0,00E+00 0,00E+00
TPE MJ 3,45E+00 2,40E-06 5,64E-03 3,45E+00
NRPE MJ 5,64E-03 8,99E-04 2,11E-02 2,76E-02
NRPM MJ 0,00E+00 0,00E+00 0,00E+00 0,00E+00
TRPE MJ 5,64E-03 8,99E-04 2,11E-02 2,76E-02
SM kg 0,00E+00 0,00E+00 0,00E+00 0,00E+00
RSF MJ 0,00E+00 0,00E+00 0,00E+00 0,00E+00
NRSF MJ 0,00E+00 0,00E+00 0,00E+00 0,00E+00
W* m3 9,86E-06 7,61E-04 3,54E-05 8,07E-04
RPEE Renewable primary energy resources used as energy carrier; RPEM Renewable primary energy
resources used as raw materials; TPE Total use of renewable primary energy resources; NRPE Non
renewable primary energy resources used as energy carrier; NRPM Non renewable primary energy
resources used as materials; TRPE Total use of non renewable primary energy resources; SM Use of
secondary materials; RSF Use of renewable secondary fuels; NRSF Use of non renewable secondary fuels; W*
Use of net fresh water. Includes evapotranspiration from reservoir.
End of life - Waste
Parameter Unit A1-A2 A3 A4 A1-A4
HW KG 1,39E-05 2,60E-09 6,86E-08 1,40E-05
NHW KG 8,18E-04 1,78E-06 3,06E-02 3,14E-02
RW KG 2,05E-08 6,47E-09 6,28E-08 8,98E-08
HW Hazardous waste disposed; NHW Non hazardous waste disposed; RW Radioactive waste disposed
End of life – output flow
Parameter Unit A1-A2 A3 A4 A1-A4
CR kg 0.00E+00 0.00E+00 0.00E+00 0.00E+00
MR kg 0.00E+00 2,79E-03 0.00E+00 2,79E-03
MER kg 0.00E+00 1,85E-06 0.00E+00 1,85E-06
EEE MJ 0.00E+00 0.00E+00 0.00E+00 0.00E+00
ETE MJ 0.00E+00 0.00E+00 0.00E+00 0.00E+00
EPD for the best environmental decision 6
CR Components for reuse; MR Materials for recycling; MER Materials for energy recovery; EEE Exported
electric energy; ETE Exported thermal energy
Reading example: 9,0 E-03 = 9,0*10-3 = 0,009
Additional environmental information
Declared unit (DU)
1 kWh electricity produced 0.9 kWh distributed to
Key environmnetal
and ready to be distributed customers
indicators
GWP – total 2,68 g CO2-eq/DU 4.49 g CO2-eq/DU
Use of primary energy 3.46 MJ/DU 3.48MJ/DU
resources
Renewable energy share 100% 99%
Energi’s hydropower plants are not located in protected areas or in protected water ways.
Their power installations and activities do not have a bigger impact on nature or society than is
Å
usual for this kind of business. Within the framework of Energi’s existing licenses, various
statutory and voluntary measures are taken to reduce the negative environmental impacts.
Å
These measures include releasing water to entice fish to swim up rivers and building salmon
ladders, putting out fish and roe in reservoirs, and actions for reduction of Eurasian eagle-owl
death by power lines ( energi 2015).
In order to reduce the Årisk of flooding in relation to the new dam constructed at Lake
Skjerkevatn, Energi is building a spillway, as well as a diversion tunnel with outlet gates to
ensure that flood water is safely diverted.
Å
Additional Norwegian requirements
Greenhous gas emission from the use of electricity in the manufacturing phase
National production mix from import, low woltage (production of transmission lines, in
addition to direct emissions and losses in grid) of applied electricity for the manufacturing
prosess(A3).
Data source Amount Unit
ecoinvent 3.7.1 (Wernet et al. 2016) 23 g CO2-eq/kWh
Dangerous substances
x The product contains no substances given by the REACH Candidate list or the
Norwegian priority list
o The product contains substances given by the REACH Candidate list or the Norwegian
priority list that are less than 0,1 % by weight.
o The product contain dangerous substances, more then 0,1% by weight, given by the
REACH Candidate List or the Norwegian Priority list, see table.
EPD for the best environmental decision 7
o The product contains no substances given by the REACH Candidate list or the
Norwegian priority list. The product is classified as hazardous waste (Avfallsforskiften,
Annex III), see table.
Indoor environment
The product does not lead to indoor emissions.
EPD for the best environmental decision 8
Bibliography
ISO 14025:2010 Environmental labels and declarations - Type III environmental
declarations - Principles and procedures
ISO 14044:2006 Environmental management - Life cycle assessment -
Requirements and guidelines
EN 15804:2012+A1:2013 Sustainability of construction works - Environmental product
declaration - Core rules for the product category of construction
products
Environdec 2021 PCR 2007:08, version 4.2. Electricity, steam and hot/cold water
generation and distribution. Date: 2021-04-26. Valid until: 2024-
03-16.
ISO 21930:2007 Sustainability in building construction - Environmental
declaration of building products
Soldal, E. 2021 Background report for the Environmental Product Declaration
for . OR.53.21. NORSUS.
Wernet et al. 2016 TheÅ e Econienrvgei nVta dnantkarbaafste version 3 (part I: overview and
methodology. The International Journal of Life Cycle Assessment
21(9: 1218-1230
Program Operator tlf +47 23 08 80 00
The Norwegian EPD Foundation
Post Box 5250 Majorstuen, 0303 Oslo e-post: post@epd-norge.no
Norway web www.epd-norge.no
Publisher tlf +47 23 08 80 00
The Norwegian EPD Foundation
Post Box 5250 Majorstuen, 0303 Oslo e-post: post@epd-norge.no
Norway web www.epd-norge.no
Owner of the decleration tlf + 47 38 60 70 00
Fax
Kjøita 18 e-post:
Å46 E3n0e Krgrii sVtaiannnskarnadft S A S web www.ae.no
oliver.germeroth@aenergi.no
Author of the life cycle assesment tlf +47 41 44 95 24
Ellen Soldal, NORSUS Fax
Stadion 4, 1671 Kråkerøy e-post: ellen@norsus.no
Norway web www.norsus.no
EPD for the best environmental decision 9
EPD for the best
environmental
decision
The Norwegian EPD foundation
www.epd-norge.no
EPD for the best environmental decision 10
