ver1 2015
ENVIRONMENTAL PRODUCT DECLARATION
in accordance with ISO 14025, ISO 21930 and EN 15804
Owner of the declaration: Jotun A/S
Program operator: The Norwegian EPD Foundation
Publisher: The Norwegian EPD Foundation
Declaration number: NEPD-2816-1513-EN
Registration number: NEPD-2816-1513-EN
ECO Platform reference number: -
Issue date: 27.04.2021
Valid to: 27.04.2026
Fenomastic Güzel Evim Zengin Mat, Jotun Boya San. ve Tic. A.S. (Turkey)
Jotun A/S
www.epd-norge.no
NEPD-2816-1513-EN Fenomastic Güzel Evim Zengin Mat, Jotun Boya San. ve Tic. A.S. (Turkey) 1 / 8
General information
Product: Owner of the declaration:
Fenomastic Güzel Evim Zengin Mat, Jotun Boya San. ve Tic. A.S. (Turkey)
Jotun A/S
Contact person: Anne Lill Gade
Phone: +47 33 45 70 00
e-mail: anne.lill.gade@jotun.no
Program operator: Manufacturer:
Jotun Boya San. ve Tic. A.S. - Paint Organize
The Norwegian EPD Foundation
Pb. 5250 Majorstuen, 0303 Oslo
Phone: +47 23 08 80 00
e-mail: post@epd-norge.no
Declaration number: Place of production:
Jotun Boya San. ve Tic. A.S. - Paint Organize
NEPD-2816-1513-EN Sanayi Bölgesi Gazi Osmanpasa Mahallesi, Ulusoy Caddesi No.6, Cerkezköy 59500
Tekirdag
Turkey
ECO Platform reference number: Management system:
ISO 9001:2008 Certificate nr: 0044915-00, ISO 14001:2004 Certificate nr 0044914-
00, ISO 45001: 2018 Certificate nr: 0098139
This declaration is based on Product Category Rules: Organisation no:
923 248 579
CEN Standard EN 15804:2012+A1:2013 serves as core PCR.
IBU PCR Part B for coatings with organic binders
Statement of liability: Issue date: 27.04.2021
The owner of the declaration shall be liable for the underlying information and
evidence. EPD Norway shall not be liable with respect to manufacturer Valid to: 27.04.2026
information, life cycle assessment data and evidences.
Declared unit: Year of study:
1 kg Fenomastic Güzel Evim Zengin Mat, Jotun Boya San. ve Tic. A.S. (Turkey) 2021
Declared unit with option: Comparability:
EPD of construction products may not be comparable if they not comply with EN
A1,A2,A3
15804 and seen in a building context.
Functional unit: Author of the Life Cycle Assessment:
The declaration is developed using EPD tool lca.tools ver EPD2020.11, developed by
LCA.no AS
Approval:
Company specific data are:
Collected/registered by: Cleo Alves Otterbech
Internal verification by: Ken Gudvangen
Verification: Approved:
Independent verification of data, other environmental information and
the declaration according to ISO14025:2010, § 8.1.3 and § 8.1.4
External
Third party verifier:
Sign
Sign
Senior Research Scientist, Anne Rønning
(Independent verifier approved by EPD Norway)
NEPD-2816-1513-EN Fenomastic Güzel Evim Zengin Mat, Jotun Boya San. ve Tic. A.S. (Turkey) 2 / 8
Product
Product description: Technical data:
Fenomastic Güzel Evim Zengin Mat is a high quality water-based paint Specific gravity: 1.38 g/cm³
which offers a rich matt appearance and natural finish. It has 100% pure Solids by volume: 33.5 ± 2 volume%
acrylic binder.
The declared product has specially designed rich matt appearance and Film thickness per coat:
natural finish, it provides an excellent color experience. Colors look richer Dry film thickness: 25 - 35 µm
and softer with their matt appearance free from the effect of brightness. It Wet film thickness: 75 - 104 µm
provides a smooth and soft appearance on the walls with its natural Theoretical spreading rate: 9.6 - 13.4 m²/l
texture.
EU limit value for the product (cat. A/a): 30 g/l. The product contains
Fenomastic Güzel Evim Zengin Mat contributes to indoor air quality with max. 21 g/l VOC.
its low VOC value. It is free from APEO and formaldehyde, and heavy
metals have not been used as active ingredients. It has low odor; so it The most representative and worst case formulation produced at the
can be applied in all seasons of the year. It has high coverage and easy manufacturing site is chosen for this EPD. For products with a selection
application properties. of colours, this will be the formulation with the highest content of
It is produced in a wide range of colours with Jotun Multicolor titanium dioxide.
Technology. Is recommended for all indoor surfaces, including residential
areas, villas and hotels. The product packaging is based on an average sized metal packaging,
including secondary packaging such as pallets and plastic wrapping.
Product specification
For information on Green Building Standard credits, see "Additional For safety, health and environmental conditions, see the Safety Data
Information" on page 4. Sheet for the declared product on www.jotun.com.
The material composition of the declared mixed product is given below: For information on technical data, application and use of the product,
see the Technical Data Sheet for the declared product on www.jotun.com.
Materials %
Water 25 - 50 % Market:
Binder 10 - 25 %
Global. Transport to market is not included in this EPD.
Filler 10 - 25 %
Reference service life, product
Titanium dioxide 10 - 25 %
The reference service life of the product is highly dependent on the
Pigment 5 - 10 %
conditions of use.
Solvents 3 - 5 %
Additive 0.3 - 1 % Estimated service life, object
Biocide <0.1% The coated object is not declared.
LCA: Calculation rules
Declared unit: Allocation:
1 kg Fenomastic Güzel Evim Zengin Mat, Jotun Boya San. ve Tic. A.S. The allocation is made in accordance with the provisions of EN 15804.
(Turkey) Incoming energy, water and waste production in-house is primarily
allocated equally among all products through mass allocation. Specific
Cut-off criteria:
allocation was performed for certain waste flows according to information
All major raw materials and essential energy is included. The production provided by the site manager. VOC emissions have been allocated
process for raw materials and energy flows with very small amounts (less entirely to the production of solvent based paints. Effects of primary
than 0.1 % dry matter) are not included. In total, more than 99% of the production of recycled materials is allocated to the main product in
material input is included. These cut-off criteria do not apply for non- which the material was used. The recycling process and transportation of
energy related emissions (such as wastes, hazardous materials and the material is allocated to this analysis.
substances).
Data quality:
The CEPE database is used as basis for the raw material composition. Specific data for the product composition and raw material amounts has been provided
by the manufacturer and represents the production of the declared product. Production site data was collected in 2015. Representative data from ecoinvent
v3.2 was used for other processes. The data quality for the material input in A1 is presented in tabular form.
Materials Source Data quality Year
Additives CEPE RM Database v3.0 Database 2016
Binders and Resins CEPE RM Database v3.0 Database 2016
Others CEPE RM Database v3.0 Database 2016
Pigments and Fillers CEPE RM Database v3.0 Database 2016
Solvents CEPE RM Database v3.0 Database 2016
Packaging Østfoldforskning Database 2017
NEPD-2816-1513-EN Fenomastic Güzel Evim Zengin Mat, Jotun Boya San. ve Tic. A.S. (Turkey) 3 / 8
System boundary:
The flowchart in the figure below illustrates the system boundaries for the analysis, in accordance with the modular principle of EN 15804. The analysis is a
cradle-to-gate (A1 - A3) study.
Additional information:
The declared product contributes to Green Building Standard credits by meeting the following specific requirements:
LEED®v4 (2013)/ LEED®v4.1 (2020)
EQ credit: Low-emitting materials
- EU/EEA/Turkey: VOC content for Interior matt walls and ceilings (Gloss <25 at 60°) WB,SB (EU Directive 2004/42/CE) and emission 0.5-5.0 mg/m³ (CDPH
method 1.2).
MR credit: Building product disclosure and optimization
- Material Ingredients, Option 2: Material Ingredient Optimization, International Alternative Compliance Path - REACH optimization: Fully inventoried chemical
ingredients to 100 ppm and not containing substances on the REACH Authorization list – Annex XIV, the Restriction list – Annex XVII and the SVHC candidate
list.
- Environmental Product Declarations. Product-specific Type III EPD (ISO 14025;21930, EN 15804) for Jotun Boya San. ve Tic. A.S. (Turkey).
BREEAM International (2016)
- Mat 01: Product-specific Type III EPD (ISO 14025;21930, EN 15804) for Jotun Boya San. ve Tic. A.S. (Turkey).
Additional certificates and approvals may be available on request.
NEPD-2816-1513-EN Fenomastic Güzel Evim Zengin Mat, Jotun Boya San. ve Tic. A.S. (Turkey) 4 / 8
LCA: Scenarios and additional technical information
The following information describe the scenarios in the different modules of the EPD.
This is a cradle to gate (A1-A3) EPD with no declared modules after the factory gate. Transport from place of production to user (A4) has to be calculated by
the user.
NEPD-2816-1513-EN Fenomastic Güzel Evim Zengin Mat, Jotun Boya San. ve Tic. A.S. (Turkey) 5 / 8
LCA: Results
System boundaries (X=included, MND=module not declared, MNR=module not relevant)
Construction Beyond the
Product stage installation User stage End of life stage . system
stage bondaries
A1 A2 A3 A4 A5 B1 B2 B3 B4 B5 B6 B7 C1 C2 C3 C4 . D
X X X MND MND MND MND MND MND MND MND MND MND MND MND MND . MND
Environmental impact
Parameter Unit A1 A2 A3
GWP kg CO 2 -eq 2,43E+00 9,84E-02 4,63E-02
ODP kg CFC11 -eq 2,26E-07 1,98E-08 2,02E-09
POCP kg C 2H 4-eq 1,26E-03 2,64E-05 1,29E-05
AP kg SO 2 -eq 1,55E-02 7,83E-04 2,62E-04
EP kg PO 3- -eq 3,63E-03 1,35E-04 3,64E-04
4
ADPM kg Sb -eq 2,54E-05 1,60E-07 3,07E-08
ADPE MJ 3,45E+01 1,62E+00 8,11E-01
GWP Global warming potential; ODP Depletion potential of the stratospheric ozone layer; POCP Formation potential of tropospheric photochemical oxidants;
AP Acidification potential of land and water; EP Eutrophication potential; ADPM Abiotic depletion potential for non fossil resources; ADPE Abiotic depletion
potential for fossil resources
Reading example: 9,0 E-03 = 9,0*10-3 = 0,009
*INA Indicator Not Assessed
waR slairetam tropsnarT gnirutcafunaM tropsnarT ylbmessA esU ecnanetniaM riapeR tnemecalpeR tnemhsibrufeR lanoitarepO ygrene esu lanoitarepO esu
retaw
-eD noitcurtsnoc noitilomed tropsnarT etsaW gnissecorp lasopsiD -yrevoceR-esueR -gnilcyceR laitnetop
NEPD-2816-1513-EN Fenomastic Güzel Evim Zengin Mat, Jotun Boya San. ve Tic. A.S. (Turkey) 6 / 8
Resource use
Parameter Unit A1 A2 A3
RPEE MJ 2,68E+00 2,68E-02 6,60E-02
RPEM MJ 5,95E-01 6,43E-03 1,16E-03
TPE MJ 3,28E+00 3,33E-02 6,71E-02
NRPE MJ 3,78E+01 1,68E+00 8,18E-01
NRPM MJ 0,00E+00 0,00E+00 0,00E+00
TRPE MJ 3,78E+01 1,68E+00 8,18E-01
SM kg 0,00E+00 0,00E+00 0,00E+00
RSF MJ 0,00E+00 0,00E+00 0,00E+00
NRSF MJ 0,00E+00 0,00E+00 0,00E+00
W m3 5,29E-02 3,44E-04 1,63E-04
RPEE Renewable primary energy resources used as energy carrier; RPEM Renewable primary energy resources used as raw materials; TPE Total use of renewable
primary energy resources; NRPE Non renewable primary energy resources used as energy carrier; NRPM Non renewable primary energy resources used as
materials; TRPE Total use of non renewable primary energy resources; SM Use of secondary materials; RSF Use of renewable secondary fuels; NRSF Use of non
renewable secondary fuels; W Use of net fresh water
Reading example: 9,0 E-03 = 9,0*10-3 = 0,009
*INA Indicator Not Assessed
End of life - Waste
Parameter Unit A1 A2 A3
HW kg 8,67E-05 7,80E-07 4,16E-07
NHW kg 1,64E+00 1,21E-01 8,67E-02
RW kg INA* INA* INA*
HW Hazardous waste disposed; NHW Non hazardous waste disposed; RW Radioactive waste disposed
Reading example: 9,0 E-03 = 9,0*10-3 = 0,009
*INA Indicator Not Assessed
End of life - Output flow
Parameter Unit A1 A2 A3
CR kg 0,00E+00 0,00E+00 0,00E+00
MR kg 0,00E+00 0,00E+00 3,34E-03
MER kg 0,00E+00 0,00E+00 8,35E-03
EEE MJ INA* INA* INA*
ETE MJ INA* INA* INA*
CR Components for reuse; MR Materials for recycling; MER Materials for energy recovery; EEE Exported electric energy; ETE Exported thermal energy
Reading example: 9,0 E-03 = 9,0*10-3 = 0,009
*INA Indicator Not Assessed
NEPD-2816-1513-EN Fenomastic Güzel Evim Zengin Mat, Jotun Boya San. ve Tic. A.S. (Turkey) 7 / 8
Additional requirements
Greenhouse gas emissions from the use of electricity in the manufacturing phase
National production mix from import, low voltage (production of transmission lines, in addition to direct emissions and losses in grid) of applied electricity for
the manufacturing process (A3).
Electricity mix Data source Amount Unit
Electricity, Turkey (kWh) ecoinvent 3.3 Alloc Rec 696,97 g CO2-ekv/kWh
Dangerous substances
The product contains no substances given by the REACH Candidate list.
Indoor environment
The declared product is emission tested by RISE Research Institutes of Sweden/SP Technical Research Institute of Sweden or Eurofins in accordance with California Department of
Public Health (CDPH) Standard Method v1.2–2017.
Bibliography
ISO 14025:2010 Environmental labels and declarations - Type III environmental declarations - Principles and procedures.
ISO 14044:2006 Environmental management - Life cycle assessment - Requirements and guidelines.
EN 15804:2012+A1:2013 Environmental product declaration - Core rules for the product category of construction products.
ISO 21930:2017 Sustainability in buildings and civil engineering works - Core rules for environmental product declarations of construction products.
IBU PCR Part B: Requirements on the EPD for Coatings with organic binders. v1.4, September 2016.
Vold et al (2017). EPD and LCA tool for Jotun - Technical description and background information, OR 01.17, Ostfold Research, Fredrikstad 2017.
CEPE v3.0 Raw materials LCI database for the European coatings and printing ink industries, May 2016.
ecoinvent v3.2 Alloc Rec, Swiss Centre of Life Cycle Inventories.
BREEAM International (2016): BREEAM International New Construction Technical Manual. SD233-2.0:2017.
EU Directive 2004/42/CE: The limitation of emissions of volatile organic compounds due to the use of organic solvents in certain paints and varnishes and vehicle refinishing
products.
CDPH method 1.2 (2017): Standard method for the testing and evaluation of volatile organic chemical emissions from indoor sources. California Department of Public Health.
LEED®v4.1 (2020): LEED® v4.1 for Building design and construction, U.S. Green Building Council®.
LEED®v4 (2013): LEED® v4 for Building design and construction, U.S. Green Building Council®.
REACH (2006): Regulation (EC) No 1907/2006 of the European Parliament and of the Council of 18 December 2006. REACH Authorization list – Annex XIV, the Restriction list –
Annex XVII and the SVHC candidate list.
Program operator and publisher Phone: +47 23 08 80 00
The Norwegian EPD Foundation e-mail: post@epd-norge.no
Post Box 5250 Majorstuen, 0303 Oslo,Norway web: www.epd-norge.no
Owner of the declaration Phone: +47 33 45 70 00
Jotun A/S e-mail: anne.lill.gade@jotun.no
Hystadveien 167 3209 Sandefjord web: www.jotun.no
Author of the Life Cycle Assessment Phone: +47 69 35 11 00
Østfoldforskning AS e-mail: post@ostfoldforskning.no
Stadion 4 1671 Kråkerøy web: www.ostfoldforskning.no
Developer of EPD generator Phone: +47 916 50 916
LCA.no AS e-mail: post@lca.no
Dokka 1C 1671 Kråkerøy web: www.lca.no
NEPD-2816-1513-EN Fenomastic Güzel Evim Zengin Mat, Jotun Boya San. ve Tic. A.S. (Turkey) 8 / 8
