ver1 2015
ENVIRONMENTAL PRODUCT DECLARATION
in accordance with ISO 14025, ISO 21930 and EN 15804
Owner of the declaration: Saint-Gobain Sweden AB, Weber floor
Program operator: The Norwegian EPD Foundation
Publisher: The Norwegian EPD Foundation
Declaration number: NEPD-2377-1110-EN
Registration number: NEPD-2377-1110-EN
ECO Platform reference number: -
Issue date: 14.09.2020
Valid to: 14.09.2025
weberfloor 4655 industry flow rapid
Saint-Gobain Sweden AB, Weber floor
www.epd-norge.no
NEPD-2377-1110-EN weberfloor 4655 industry flow rapid 1 / 8
General information
Product: Owner of the declaration:
weberfloor 4655 industry flow rapid Saint-Gobain Sweden AB, Weber floor
Contact person: Anders Anderberg
Phone: +46 8 625 6105
e-mail: anders.anderberg@weber.se
Program operator: Manufacturer:
The Norwegian EPD Foundation Saint-Gobain Sweden AB, Weber floor
Pb. 5250 Majorstuen, 0303 Oslo
Phone: +47 23 08 80 00
e-mail: post@epd-norge.no
Declaration number: Place of production:
Saint-Gobain Sweden AB, Weber, Vingåker
NEPD-2377-1110-EN
ECO Platform reference number: Management system:
ISO 9001, ISO 14001
This declaration is based on Product Category Rules: Organisation no:
SE-556241-2592
CEN Standard EN 15804:2012+A1:2013 serves as core PCR.
Statement of liability: Issue date: 14.09.2020
The owner of the declaration shall be liable for the underlying information and
evidence. EPD Norway shall not be liable with respect to manufacturer Valid to: 14.09.2025
information, life cycle assessment data and evidences.
Declared unit: Year of study:
1 kg weberfloor 4655 industry flow rapid 2019
Declared unit with option: Comparability:
EPD of construction products may not be comparable if they not comply with EN
A1,A2,A3,A4,A5
15804 and seen in a building context.
Functional unit: Author of the Life Cycle Assessment:
The declaration is developed using eEPD v4.0 from LCA.no
Approval:
Company specific data are:
Collected/registered by: Thomas Flycht
Internal verification by: Helene Wallgren
Verification: Approved:
Independent verification of data, other environmental information and the
declaration according to ISO14025:2010, § 8.1.3 and § 8.1.4
External
Third party verifier:
Sign Sign
Senior Research Scientist, Anne Rønning
(Independent verifier approved by EPD Norway)
NEPD-2377-1110-EN weberfloor 4655 industry flow rapid 2 / 8
Product
Product description: Technical data:
Weberfloor 4655 super flow rapid is a pumpable rapid hardening self- weberfloor 4655 industry flow rapid is designed, produced and CE marked
levelling compound for floors internally in buildings with light industrial according to EN 13813
loads such as industrial areas, public areas, basements and storage
rooms. It is ready for traffic loads without further finishing, but can also For further information, see www.se.weber/
be used as a substrate for resin flooring.
Market:
Product specification
Scandinavian countries
The composition of the product is described in the following table:
Reference service life, product
Materials %
>50 years
Binder 15-40
Aggregate 20-60 Reference service life, building
Filler 10-30
>50 years
Additives 1-5
LCA: Calculation rules
Declared unit: Allocation:
The allocation is made in accordance with the provisions of EN 15804.
1 kg weberfloor 4655 industry flow rapid
Incoming energy and water and waste production in-house is allocated
Cut-off criteria: equally among all products through mass allocation. Effects of primary
production of recycled materials is allocated to the main product in which the
All major raw materials and all the essential energy is included. The
material was used. The recycling process and transportation of the material is
production processes for raw materials and energy flows with very small
allocated to this analysis.
amounts (less than 1%) are not included. These cut-off criteria do not
apply for hazardous materials and substances.
Data quality:
Specific data for the product composition are provided by the manufacturer. They represent the production of the declared product and were collected for EPD
development in the year of study. Background data is based on registered EPDs according to EN 15804, Ostfold Research databases, ecoinvent and other LCA
databases. The data quality of the raw materials in A1 is presented in the table below.
Materials Source Data quality Year
Cement Supplier EPD 2012
Binder EPD-BVG-20140073-IAG1-EN EPD 2014
Cement Supplier EPD 2014
Additives ecoinvent 3.4 Database 2017
Aggregate ecoinvent 3.4 Database 2017
Filler ecoinvent 3.4 Database 2017
NEPD-2377-1110-EN weberfloor 4655 industry flow rapid 3 / 8
System boundary:
All processes from raw material extraction to product transport to the construction site and assembly are included in the analysis (A1-A5). The flow chart below
illustrates the system boundaries for the A1 to A3 part of the analysis.
Additional technical information:
The consumption of the product is 1,7 kg / m² / mm.
The remaining powder and cured material may be disposed as construction waste to disposal or recycling.
NEPD-2377-1110-EN weberfloor 4655 industry flow rapid 4 / 8
LCA: Scenarios and additional technical information
The following information describe the scenarios in the different modules of the EPD.
Transport to market (A4) is calculated based on the default distance of 300 km from NPCR 012
Transport from production place to user (A4)
Capacity utilisation Fuel/Energy
Type Type of vehicle Distance km Unit Value (l/t)
(incl. return) % consumption
Truck 55,0 % Truck, lorry over 32 tonnes, EURO 5 300 0,022823 l/tkm 6,85
Railway l/tkm
Boat l/tkm
Other Transportation l/tkm
Additional A4 information Unit/Range Value
Multiplication factor
Lilleström, Norway (truck / truck to jobsite: 677 km) 1,65
GWP/A4
Multiplication factor
Karlslunde, Denmark (truck / truck to jobsite: 885 km) 2,02
GWP/A4
Multiplication factor
Helsinki, Finland (truck / roro boat / truck to jobsite: 952 km) 2,13
GWP/A4
Assembly (A5)
. Unit Value
Auxiliary kg
Water consumption m3 0,0002
Electricity consumption kWh 0,0021
Other energy carriers MJ
Material loss kg
Output materials from waste treatment kg 0,0000
Dust in the air kg
VOC emissions kg
NEPD-2377-1110-EN weberfloor 4655 industry flow rapid 5 / 8
LCA: Results
System boundaries (X=included, MND=module not declared, MNR=module not relevant)
Construction Beyond the
Product stage installation User stage End of life stage . system
stage bondaries
A1 A2 A3 A4 A5 B1 B2 B3 B4 B5 B6 B7 C1 C2 C3 C4 . D
X X X X X MND MND MND MND MND MND MND MND MND MND MND . MND
Environmental impact
Parameter Unit A1-A3 A4 A5
GWP kg CO 2 -eq 2,58E-01 2,62E-02 1,77E-04
ODP kg CFC11 -eq 2,37E-08 5,10E-09 1,07E-10
POCP kg C 2H 4-eq 6,15E-05 4,23E-06 5,13E-08
AP kg SO 2 -eq 1,03E-03 8,51E-05 9,43E-07
EP kg PO 3- -eq 1,57E-04 1,43E-05 1,74E-07
4
ADPM kg Sb -eq 2,11E-06 5,91E-08 1,48E-09
ADPE MJ 3,44E+00 4,11E-01 1,68E-03
GWP Global warming potential; ODP Depletion potential of the stratospheric ozone layer; POCP Formation potential of tropospheric photochemical oxidants;
AP Acidification potential of land and water; EP Eutrophication potential; ADPM Abiotic depletion potential for non fossil resources; ADPE Abiotic depletion
potential for fossil resources
"Reading example: 9,0 E-03 = 9,0*10-3 = 0,009"
*INA Indicator Not Assessed
waR slairetam tropsnarT gnirutcafunaM tropsnarT ylbmessA esU ecnanetniaM riapeR tnemecalpeR tnemhsibrufeR lanoitarepO ygrene esu lanoitarepO esu
retaw
-eD noitcurtsnoc noitilomed tropsnarT etsaW gnissecorp lasopsiD -yrevoceR-esueR -gnilcyceR laitnetop
NEPD-2377-1110-EN weberfloor 4655 industry flow rapid 6 / 8
Resource use
Parameter Unit A1-A3 A4 A5
RPEE MJ 3,40E-01 7,42E-03 5,97E-03
RPEM MJ 0,00E+00 0,00E+00 0,00E+00
TPE MJ 3,40E-01 7,42E-03 5,97E-03
NRPE MJ 3,94E+00 4,23E-01 1,46E-02
NRPM MJ 0,00E+00 0,00E+00 0,00E+00
TRPE MJ 3,94E+00 4,23E-01 1,46E-02
SM kg 6,84E-02 0,00E+00 0,00E+00
RSF MJ 1,69E-02 0,00E+00 5,60E-06
NRSF MJ 5,61E-01 0,00E+00 0,00E+00
W m3 1,64E-03 9,98E-05 2,84E-04
RPEE Renewable primary energy resources used as energy carrier; RPEM Renewable primary energy resources used as raw materials; TPE Total use of renewable
primary energy resources; NRPE Non renewable primary energy resources used as energy carrier; NRPM Non renewable primary energy resources used as
materials; TRPE Total use of non renewable primary energy resources; SM Use of secondary materials; RSF Use of renewable secondary fuels; NRSF Use of non
renewable secondary fuels; W Use of net fresh water
"Reading example: 9,0 E-03 = 9,0*10-3 = 0,009"
*INA Indicator Not Assessed
End of life - Waste
Parameter Unit A1-A3 A4 A5
HW kg 9,75E-06 2,25E-07 8,57E-09
NHW kg 5,66E-02 3,84E-02 1,78E-04
RW kg INA* INA* INA*
HW Hazardous waste disposed; NHW Non hazardous waste disposed; RW Radioactive waste disposed
"Reading example: 9,0 E-03 = 9,0*10-3 = 0,009"
*INA Indicator Not Assessed
End of life - Output flow
Parameter Unit A1-A3 A4 A5
CR kg 0,00E+00 0,00E+00 0,00E+00
MR kg 0,00E+00 0,00E+00 0,00E+00
MER kg 3,00E-04 0,00E+00 0,00E+00
EEE MJ INA* INA* INA*
ETE MJ INA* INA* INA*
CR Components for reuse; MR Materials for recycling; MER Materials for energy recovery; EEE Exported electric energy; ETE Exported thermal energy
"Reading example: 9,0 E-03 = 9,0*10-3 = 0,009"
*INA Indicator Not Assessed
NEPD-2377-1110-EN weberfloor 4655 industry flow rapid 7 / 8
Additional Norwegian requirements
Greenhouse gas emissions from the use of electricity in the manufacturing phase
National production mix from import, low voltage (production of transmission lines, in addition to direct emissions and losses in grid) of applied electricity for the
manufacturing process (A3).
Electricity mix Data source Amount Unit
Renewable electricity with Guarantee of Origin from LOS (kWh) Modified ecoinvent 3.4 60,20 g CO2-ekv/kWh
Dangerous substances
The product contains no substances given by the REACH Candidate list or the Norwegian priority list.
Name CASNo Amount
Portland Cement 65997-15-1 2-5%
Indoor environment
Bibliography
ISO 14025:2010 Environmental labels and declarations - Type III environmental declarations - Principles and procedures.
ISO 14044:2006 Environmental management - Life cycle assessment - Requirements and guidelines.
EN 15804:2012+A1:2013 Environmental product declaration - Core rules for the product category of construction products.
ISO 21930:2017 Sustainability in buildings and civil engineering works. Core rules for environmental product declarations of construction products.
ecoinvent v3, Allocation, cut-off by classification, Swiss Centre of Life Cycle Inventories.
Iversen et al., (2018) eEPD v3.0 - Background information for EPD generator system, LCA.no report number 04.18
Iversen et al., (2019) EPD generator for Saint-Gobain Weber and Scanspac - Background information and LCA data, LCA.no report number 05.18
NPCR Part A: Construction products and services. Ver. 1.0. April 2017, EPD-Norge.
NPCR 009 Part B for technical-chemical products. Ver. 1.0 June 2018, EPD-Norge.
Program operator and publisher Phone: +47 23 08 80 00
The Norwegian EPD Foundation
Post Box 5250 Majorstuen, 0303 Oslo e-mail: post@epd-norge.no
0303 Oslo Norway web: www.epd-norge.no
Owner of the declaration Phone: +46 8 625 6105
Saint-Gobain Sweden AB, Weber floor Fax:
Box 415 e-mail: anders.anderberg@weber.se
SE-19162 Sollentuna web: www.weber.se
Author of the Life Cycle Assessment Phone: +47 916 50 916
LCA.no AS Fax: 90571091
Dokka 1C e-mail: post@lca.no
1671 Kråkerøy web: www.lca.no
Developer of EPD generator Phone: +47 916 50 916
LCA.no AS
Dokka 1C e-mail: post@lca.no
1671 Kråkerøy web: www.lca.no
NEPD-2377-1110-EN weberfloor 4655 industry flow rapid 8 / 8
