Environmental Product Declaration:
Norlite Perlite, fire-proof thermal
insulation
In accordance with ISO 14025 and EN 15804 +A2
Owner of the declaration: Product name
Nordisk Perlite ApS
Norlite Perlite, fire-proof
Program holder and publisher:
thermal insulation
The Norwegian EPD foundation
Declaration number:
Manufacturer
Nordisk Perlite ApS
NEPD-3654-2600-EN
Registration Number:
]
NIsEsPuDe- d3a6t5e4: -2600-EN
Valid to: 03.08.2022
The Norwegian
03.08.2027
EPD Foundation
General information
Product: Owner of the declaration:
Norlite Perlite 0515 SC, 0530 SC and 0560 SC Nordisk Perlite ApS
Contact person: Cees Vader
Program Operator: Phone: 0045 78789521
e-mail: cees@nordiskperlite.dk
The Norwegian EPD Foundation
Post Box 5250 Majorstuen, 0303 Oslo, Norway
Tlf: +47 23 08 80 00 Manufacturer:
e-mail: post@epd-norge.no Nordisk Perlite ApS
Hammersholt Erhvervspark 1-5
Declaration Number: DK-3400 Hillerød, Denmark
Phone: +45 48 14 07 22
e-mail: nordisk@perlite.dk
NEPD-3654-2600-EN
This declaration is based on Product
Place of production:
Category Rules:
Hammersholt, Denmark
EN 15804:2012+A2:2019 and c-PCR EN 16783
Management system:
Statements:
ISO 9001
The owner of the declaration shall be liable for the
underlying information and evidence. EPD
Organisation no:
Norway shall not be liable with respect to
DK48247717
manufacturer, life cycle assessment data and
evidences.
Issue date:
Declared unit:
1 m3 of Norlite Perlite
03.08.2022
Valid to:
Declared unit with option:
1 m3 of Norlite Perlite
03.08.2027
Year of study:
A1-A5, B1-B7, C1-C4 and D
2021
Functional unit:
Comparability:
1 m3 of Norlite Perlite with bulk density 85 kg/m³
EPDs from other programmes than EPD Norway
with insulation value of 0,042 W/m.K
may not be comparable.
Verification:
Independent verification of the declaration and The EPD has been worked out by:
data, according to ISO14025:2010 Amy Stockwell, Eando AB
amy.stockwell@eando.se
internal external X
X
Silvia Vilčeková
Independent verifier approved by EPD Norway Approved (Manager of EPD Norway)
EPD for the best environmental decision 2
Product
Product description:
Norlite Perlite 0515 SC, 0530 SC and 0560 SC are expanded perlite aggregates. The raw perlite
is expanded 10 – 15 times in size in a furnace, at 1000°C, driven by natural gas. All SC-products
are coated with a special water-proof membrane, preventing water and humidity from
penetrating and have a capillary breaking height of 4 cm. Nordisk Perlite produces 3 different
particle sizes, that all can be used for thermal insulation, with a value of 0.042 W/m.K. Norlite
Perlite 0515 SC, 0530 SC and 0560 SC is a loose fill insulation tested according to DS/EN
12667:2001 and DS/EN 15501:2013. Other applications are light weight hydrophobic filler and
selective absorber of oils.
Norlite Perlite 0515 SC, 0530 SC and 0560 SC has 0 % VOC as the product exists of a mineral
with a polymeric coating; the polymeric siloxane is chemically bound to the perlite mineral.
Norlite Perlite 0515 SC, 0530 SC and 0560 SC does not need a safety datasheet as the product
has no health and safety sentences. It is therefore safe to use for all applications.
Norlite Perlite 0515 SC, 0530 SC and 0560 SC is used for floor, wall and roof insulation, shows
noise absorption properties and forms a natural fire-proof layer, A1 in fire-class in all
applications. Norlite Perlite 0515 SC, 0530 SC and 0560 SC are among the lightest mineral
aggregates on the market.
Correctly installed, Norlite Perlite 0515 SC, 0530 SC and 0560 SC will last forever as insulation
material as the products do not absorb water, are heat-, cold- and dimension-stable.
Product specification:
Norlite Perlite 0515 SC, 0530 SC and 0560 SC are produced by expanding raw perlite with
natural gas in a furnace, hereafter the expanded grades 0515, 0530 and 0560 are treated with a
siloxane and become the hydrophobic grades 0515 SC, 0530 SC and 0560 SC. Norlite Perlite
0515 SC, 0530 SC and 0560 SC are REACH exempt.
Materials kg per m3 %
Perlite 84.75 – 84.83 99.7 – 99.8
Siloxane 0.17 – 0.25 0.2 – 0.3
Technical data:
Norlite Perlite Expand comes in 3 sizes: 0515 SC (0,5-1,5 mm), 05 30 SC (0,5 – 3,0 mm) and 05
60 SC (0,5 -6,0 mm). All have a bulk density of 85 kg/m³ and an insulation value of 0.042
W/m.K
Market:
Europe
Reference service life, product:
Equal to the building service life, of at least 50 years.
Reference service life, building:
Equal to the building service life
EPD for the best environmental decision 3
Declared unit:
1m3 of siloxane coated Norlite Perlite for building insulation, including A1-A5, B1-B7, C1-C4 and
D.
Data quality:
The manufacturing process A3 is based on specific 2021 total production data obtained from
Nordisk Perlite. Transportation data A2 was also provided by Nordisk Perlite. Some data was
provided from a Turkish perlite mine, which was inserted into the Ecoinvent perlite quarry
operation dataset. Other raw materials in A1 use generic data from GaBi and Ecoinvent datasets
shown in the LCA scenarios section.
Allocation:
No allocation was required for the manufacturing of perlite. All expanded perlite is sold in a
variety of formats. For example the perlite which cannot be used for insulation or filtration, is
used as sterile underlay in cattle sheds. The energy required for coating is recorded separately
to that of expansion, so no allocation required.
System boundary:
All life cycle stages are included in the study: product stage (A1-A3), construction process (A4-
A5), end of life (module C) and module D. Module B is not associated with any activities or
emissions causing any environmental impacts.
Benefits
& loads
Assembly
Product stage Use stage End of life stage beyond
stage
system
boundary
EPD for the best environmental decision 4
slairetam
waR
tropsnarT
gnirutcafunaM
tropsnarT ylbmessA
esU
ecnanetniaM
riapeR
tnemecalpeR
tnemhsibrufeR
esu
ygrene
lanoitarepO
esu
retaw
lanoitarepO
noitilomed
noitcurtsnoc-eD
tropsnarT
gnissecorp
etsaW
lasopsiD
-gnilcyceR-yrevoceR-esueR
laitnetop
LCA: Calculation rules
Module A1 A2 A3 A4 A5 B1 B2 B3 B4 B5 B6 B7 C1 C2 C3 C4 D
Module
X X X X X X X X X X X X X X X X X
declared
Geography TR/EU EU DK DK DK ND ND ND ND ND ND ND DK DK DK DK DK
A1, raw material supply
This module considers the extraction and processing of all raw materials, energy, and
transportation which occur upstream to the studied manufacturing process, including
packaging material (except for ancillary material used in product manufacturing process).
A2, transport to the manufacturer
The raw materials are transported to the manufacturing site. This also includes coatings and
packaging material.
A3, manufacturing
This module includes manufacturing of expanded perlite and the coating of it for the following
products:
Norlite Perlite 0515 SC
Norlite Perlite 0530 SC
Norlite Perlite 0560 SC
A4-A5 Construction process stage
A4, Transport
Transportation from Nordisk Perlite to the building site is taken into account.
A5, Construction installation
This stage includes any resources used during the installation of the product on the
construction site. In this case the insulation can either be installed manually (no emissions) or
by blower. Waste is negligible as perlite does not need to be cut into shape. 1% waste was
assumed as spillage and dust and that it would be in quantities too small to be recycled.
Treatment of the packaging waste on site is considered and assumes average Danish end of life
rates for mixed construction waste.
B Use stage
B1-B7
This stage includes no activities or emissions related to the product.
C End of life stage
Norlite Perlite 0515 SC, 0530 SC and 0560 SC can be re-used, either as insulation, with the same
properties as virgin perlite, or be used in concrete as light weight filler.
C1 Deconstruction/Demolition
Norlite Perlite 0515 SC, 0530 SC and 0560 SC can easily be collected by gathering the material
in big bags through suction. This requires the same amount of energy and same type of
equipment as to install the perlite. Therefore the values of C1 are the same as A5. Of course
other methods to gather Norlite Perlite 0515 SC, 0530 SC and 0560 SC can be used, but these
are not documented in this EPD. It is assumed that all perlite will be collected for reuse.
C2 Transport
Transport distance to waste processing for mixed construction waste.
C3 Waste processing
All Norlite Perlite can be reused in section D. Mixed construction waste follows Danish average
values.
C4 Final disposal
All Norlite Perlite can be reused in section D. Mixed construction waste follows Danish average
values.
D Benefits and loads beyond the system boundary
Emission credits are obtained from the reuse of perlite as a concrete filler, at the end of the life
of the building.
At the manufacturing phase heat energy is recovered and used as local heating. It is assumed to
be a substitute for thermal energy from natural gas. Much of the packaging is made from mono-
materials which can be recycled and credited here.
EPD for the best environmental decision 5
Cut-off criteria:
All input and output flows in a unit process were considered i.e., taking into account the value of
all flows in the unit process and the corresponding LCI where data was available. Data gaps
were filled by conservative assumptions with average or generic data. Any assumptions in such
case were documented. The use of cut-off criterion on mass inputs and primary energy at the
unit process level (1%) and at the information module level (5%).
LCA: Scenarios and additional technical information
The following information describe the scenarios in the different modules of the EPD.
Raw materials: perlite mining and siloxane (A1)
Some data was provided from the Turkish perlite mines. This was inserted into the Ecoinvent
dataset on perlite quarry operation.
Materials Source Data quality Year Geography
Diesel, mix at filling station
Sphera Database 2018 EU28
Electricity, high voltage production mix
Ecoinvent 3.8 Database 2018 TR
Lubricants at refinery Sphera Database 2018 EU28
Market for mine infrastructure,
Ecoinvent 3.8 Database 2011 GLO
vermiculite
2000 with
Perlite quarry operation Ecoinvent 3.8 Database DE
updates
Polydimethylsiloxane, market for Ecoinvent 3.8 Database 2015 GLO
Tap water from ground water Sphera Database 2020 EU28
Thermal energy from heavy fuel oil
Sphera Database 2018 GR
The mine infrastructure dataset is old, but there was no other data available. Analysis was
completed to show its impact on the total environmental impact was negligible (maximum of
0.28%) for all of the main impact indicators.
Transport from production place to assembly/user (A4)
Fuel/Energy
Type Capacity utilisation % Type of vehicle Distance km
consumption
Truck 28% Truck trailer with 27t payload 250 0.0167 kg/tkm
This distance is estimated based on knowledge of consumer locations. Perlite once expanded is
a very low density at 85 kg/m3, so one truck can carry only 7.65 tonnes, which is unusually low.
Fuel type Source Data quality Year
EU 28: Diesel mix (6,35% bio-content) Sphera Database 2017
EPD for the best environmental decision 6
Assembly (A5)
Unit Value /m3
Electricity consumption kWh 0.018
Material loss % 1
Perlite can either be installed manually (no energy required) or by blow machine. The same
amount of waste is assumed for each.
Use Stage(B)
B1-B7: Perlite is stable and inert. Therefore there are no environmental impacts expected in the
use phase and no harmful substances are released to air, water or ground during the use of the
product.
End of Life (C1, C3, C4)
Norlite Perlite 0515 SC, 0530 SC and 0560 SC can be re-used, either as insulation, showing the
same parameters as new product, or be used in concrete as light weight filler. The method to
remove Norlite Perlite 0515 SC, 0530 SC and 0560 SC documented in this EPD is to gather the
material in big bags through suction. This requires the same amount of energy and same type of
equipment as to install the perlite by blowing it in place. Therefore the values of C1 are the
same as A5. Other methods to gather Norlite Perlite 0515 SC, 0530 SC and 0560 SC can be used,
but these are not documented in this EPD.
Nordisk Perlite we work for circular economic products. This criteria Norlite Perlite 0515 SC,
0530 SC and 0560 SC can fulfill by reuse or use as light weight filler in concrete. Therefore
disposal is only considered for waste during construction phase (ie dust and spillage).
Transport to waste processing (C2)
Fuel/Energy
Type Capacity utilisation (incl. return) % Type of vehicle Distance km
consumption
Truck 61% Truck trailer 100 0.0167 kg/tkm
Transportation distance to waste processing facility is assumed to be 100km
Benefits and loads beyond the system boundaries (D)
Norlite Perlite 0515 SC, 0530 SC and 0560 SC can be reused, fulfilling the circular economic
criteria of using the product as intended when producing the virgin product, we have a cradle-
to-cradle application.
Norlite Perlite 0515 SC, 0530 SC and 0560 SC can be used as light weight filler in concrete. A
known problem in the concrete industry is the need for light and good quality aggregates. As it
might not be possible to reuse Norlite Perlite 0515 SC, 0530 SC and 0560 SC as insulation in all
cases, we have documented this solution. Concrete cubes were made according to DS/EN 206-9
NA: 5 cubes per formulation of Concrete 35. In the table below, the average results are
presented. Weight reduction can be achieved, but the strength of the concrete should be
observed. Larger amounts of Norlite Perlite 05 15 SC, 05 30 SC and 05 60 SC can be added to
concrete, but this was not tested at the time. In the test 0.1 and 0.25 % of sand were replaced
by Norlite Perlite 05 60 SC on a 1:1 weight basis. Type 05 60 SC was used as this is the mostly
used insulation type.
EPD for the best environmental decision 7
Compressive Compressive Weight Density
Sample
Strength (kN) Strength (MPa) Cube (kg) (kg/m³)
Concrete 35 reference 772 34.31 7.22 2139
Concrete 35 + 0,1 % Norlite Perlite 05
628 27.91 7.20 2131
60 SC
Concrete 35 + 0,25 % Norlite Perlite 05
568 25.24 6.96 2062
60 SC
As noted in section A3, waste heat is used as district heating for which there is credit. Recycled
and incinerated packaging materials also gain credits here.
Per m3 perlite Unit Value
Waste heat that substitutes natural gas in a district heating plan kWh 41.5
Perlite replacing concrete kg 85
Electricity from incinerating waste perlite kWh -0.67
Thermal energy from incinerating waste perlite kWh -0.17
Recycled polypropylene produced kg 0.84
Electricity from packaging disposal kWh 0.58
Thermal energy from packaging disposal kWh 1.00
Recycled HDPE produced kg 0.19
Additional technical information
Nordisk Perlite is a supplier of perlite products for many different applications; from filtration
to horticulture to insulation. The products are all based on expanded perlite. The insulation
products have an indefinite service life and require no maintenance during use. Norlite Perlite
0515 SC, 0530 SC and 0560 SC can be reused either for new insulating jobs or as light weight
aggregate in concrete.
EPD for the best environmental decision 8
System boundaries (X=included)
Benefits
& loads
Assembly
Product stage Use stage End of life stage beyond
stage
system
boundary
EPD for the best environmental decision 9
slairetam
waR
tropsnarT
gnirutcafunaM
tropsnarT ylbmessA
esU
ecnanetniaM
riapeR
tnemecalpeR tnemhsibrufeR
esu
ygrene
lanoitarepO
esu
retaw
lanoitarepO
noitilomed
noitcurtsnoc-eD
tropsnarT
gnissecorp
etsaW
lasopsiD
-gnilcyceR-yrevoceR-esueR
laitnetop
LCA: Results
A1 A2 A3 A4 A5 B1 B2 B3 B4 B5 B6 B7 C1 C2 C3 C4 D
X X X X X X X X X X X X X X X X X
Core environmental impact indicators
Indicator Unit A1-A3 A4 A5 B C1 C2 C3 C4 D
GWP-total kg CO2 eq.
2.09E+01 2.38E+00 2.48E-01 0 4.75E-03 5.12E-01 6.03E-01 0 -7.86E+00
GWP-fossil kg CO2 eq.
2.08E+01 2.37E+00 2.44E-01 0 4.73E-03 5.10E-01 5.76E-01 0 -7.85E+00
GWP-
kg CO2 eq.
biogenic 1.81E-02 -3.25E-03 4.26E-03 0 2.22E-05 -7.00E-04 2.59E-02 0 -6.90E-03
GWP-
kg CO2 eq.
LULUC 1.19E-02 1.31E-02 9.05E-05 0 1.68E-06 2.83E-03 1.14E-03 0 -5.79E-03
kg CFC11
ODP
eq. 1.48E-04 1.41E-13 7.18E-10 0 8.25E-14 3.04E-14 5.33E-09 0 -1.21E-11
AP mol H⁺ eq.
2.35E-01 5.03E-03 4.63E-04 0 7.50E-06 9.51E-04 2.31E-03 0 -1.47E-02
EP-
kg P eq.
freshwater 1.28E-03 7.02E-06 1.23E-06 0 2.69E-08 1.51E-06 1.15E-06 0 -5.81E-06
EP-marine kg N eq.
5.79E-02 2.16E-03 1.63E-04 0 2.54E-06 3.96E-04 9.30E-04 0 -4.86E-03
EP-
mol N eq.
terrestrial 6.33E-01 2.44E-02 1.65E-03 0 2.48E-05 4.50E-03 1.02E-02 0 -5.33E-02
kg NMVOC
POCP
eq. 1.64E-01 4.54E-03 4.06E-04 0 6.06E-06 8.52E-04 2.54E-03 0 -1.37E-02
ADP-M&M kg Sb eq.
1.59E-05 1.97E-07 1.14E-07 0 2.51E-09 4.24E-08 2.89E-07 0 -3.41E-07
ADP-fossil MJ
3.04E+02 3.14E+01 2.92E+00 0 5.67E-02 6.77E+00 9.47E+00 0 -4.50E+01
WDP m³
2.92E+00 2.11E-02 5.82E-02 0 3.98E-04 4.55E-03 3.74E-01 0 -5.74E-01
GWP-total: Global Warming Potential; GWP-fossil: Global Warming Potential fossil fuels; GWP-biogenic:
Global Warming Potential biogenic; GWP-LULUC: Global Warming Potential land use and land use change;
ODP: Depletion potential of the stratospheric ozone layer; AP: Acidification potential, Accumulated
Exceedance; EP-freshwater: Eutrophication potential, fraction of nutrients reaching freshwater end
compartment; See “additional Norwegian requirements” for indicator given as PO4 eq. EP-marine:
Eutrophication potential, fraction of nutrients reaching freshwater end compartment; EP-terrestrial:
Eutrophication potential, Accumulated Exceedance; POCP: Formation potential of tropospheric ozone; ADP-
M&M: Abiotic depletion potential for non-fossil resources (minerals and metals); ADP-fossil: Abiotic
depletion potential for fossil resources; WDP: Water deprivation potential, deprivation weighted water
consumption
Additional environmental impact indicators
Indicator Unit A1-A3 A4 A5 B C1 C2 C3 C4 D
Disease
PM
incidence 3.51E-06 2.69E-08 4.38E-09 0 6.76E-11 5.32E-09 3.33E-08 0 -1.91E-07
IRP kBq U235 eq.
2.79E-01 5.68E-03 2.40E-02 0 5.24E-04 1.23E-03 8.17E-02 0 -4.02E-01
ETP-fw CTUe
6.09E+02 2.18E+01 3.62E+00 0 1.93E-02 4.70E+00 2.45E+01 0 -2.28E+01
HTP-c CTUh
5.02E-09 4.40E-10 9.63E-11 0 1.92E-12 9.48E-11 1.55E-10 0 -1.01E-09
HTP-nc CTUh
1.34E-07 2.41E-08 3.06E-09 0 4.23E-11 5.16E-09 1.20E-08 0 -1.03E-07
SAP Dimensionless
-3.01E+01 1.08E+01 3.76E+00 0 8.26E-02 2.33E+00 2.04E+00 0 -9.92E+00
PM: Particulate matter emissions; IRP: Ionising radiation, human health; ETP-fw: Ecotoxicity (freshwater);
ETP-c: Human toxicity, cancer effects; HTP-nc: Human toxicity, non-cancer effects; SQP: Land use related
impacts / soil quality
Classification of disclaimers to the declaration of core and additional environmental
impact indicators
ILCD classification Indicator Disclaimer
Global warming potential (GWP) None
ILCD type / level 1 Depletion potential of the stratospheric ozone layer (ODP) None
Potential incidence of disease due to PM emissions (PM) None
Acidification potential, Accumulated Exceedance (AP) None
Eutrophication potential, Fraction of nutrients reaching freshwater end
None
compartment (EP-freshwater)
Eutrophication potential, Fraction of nutrients reaching marine end
None
compartment (EP-marine)
ILCD type / level 2
Eutrophication potential, Accumulated Exceedance (EP-terrestrial) None
Formation potential of tropospheric ozone (POCP) None
Potential Human exposure efficiency relative to U235 (IRP) 1
Abiotic depletion potential for non-fossil resources (ADP-minerals&metals) 2
Abiotic depletion potential for fossil resources (ADP-fossil) 2
Water (user) deprivation potential, deprivation-weighted water
2
consumption (WDP)
ILCD type / level 3 Potential Comparative Toxic Unit for ecosystems (ETP-fw) 2
Potential Comparative Toxic Unit for humans (HTP-c) 2
Potential Comparative Toxic Unit for humans (HTP-nc) 2
Potential Soil quality index (SQP) 2
Disclaimer 1 – This impact category deals mainly with the eventual impact of low dose ionizing radiation on
human health of the nuclear fuel cycle. It does not consider effects due to
possible nuclear accidents, occupational exposure nor due to radioactive waste disposal in underground facilities.
Potential ionizing radiation from the soil, from radon and from some
construction materials is also not measured by this indicator.
Disclaimer 2 – The results of this environmental impact indicator shall be used with care as the uncertainties on
these results are high or as there is limited experienced with the indicator
EPD for the best environmental decision 10
Resource use
Indicator Unit A1-A3 A4 A5 B C1 C2 C3 C4 D
RPEE MJ 3.31E+01 1.79E+00 5.42E+00 0 1.20E-01 3.85E-01 1.82E+00 0 -9.05E+00
RPEM MJ 2.85E+00 0.00E+00 0.00E+00 0 0.00E+00 0.00E+00 0.00E+00 0 0.00E+00
TPE MJ 3.31E+01 1.79E+00 5.42E+00 0 1.20E-01 3.85E-01 1.82E+00 0 -9.05E+00
NRPE MJ 3.04E+02 3.15E+01 2.92E+00 0 5.67E-02 6.79E+00 9.48E+00 0 -4.51E+01
NRPM MJ 4.48E+01 0.00E+00 0.00E+00 0 0.00E+00 0.00E+00 0.00E+00 0 0.00E+00
TRPE MJ 3.04E+02 3.15E+01 2.92E+00 0 5.67E-02 6.79E+00 9.48E+00 0 -4.51E+01
SM kg 0.00E+00 0.00E+00 0.00E+00 0 0.00E+00 0.00E+00 0.00E+00 0 0.00E+00
RSF MJ 0.00E+00 0.00E+00 0.00E+00 0 0.00E+00 0.00E+00 0.00E+00 0 3.74E-02
NRSF MJ 0.00E+00 0.00E+00 0.00E+00 0 0.00E+00 0.00E+00 0.00E+00 0 1.46E-01
W m3 7.59E-02 2.02E-03 2.82E-03 0 4.15E-05 4.35E-04 9.57E-03 0 -1.77E-02
RPEE Renewable primary energy resources used as energy carrier; RPEM Renewable primary energy
resources used as raw materials; TPE Total use of renewable primary energy resources; NRPE Non-
renewable primary energy resources used as energy carrier; NRPM Non-renewable primary energy
resources used as materials; TRPE Total use of non-renewable primary energy resources; SM Use of
secondary materials; RSF Use of renewable secondary fuels; NRSF Use of non-renewable secondary fuels; W
Use of net fresh water
End of life - Waste
Indicator Unit A1-A3 A4 A5 B C1 C2 C3 C4 D
HW kg 1.31E-08 1.51E-10 6.37E-10 0 1.37E-11 3.25E-11 3.89E-10 0 -1.51E-09
NHW kg 1.28E-01 4.51E-03 5.28E-01 0 1.92E-04 9.73E-04 3.30E+00 0 -2.56E+00
RW kg 1.15E-03 3.88E-05 2.26E-04 0 4.72E-06 8.36E-06 5.65E-04 0 -2.38E-03
HW Hazardous waste disposed; NHW Non-hazardous waste disposed; RW Radioactive waste disposed
End of life – output flow
Indicator Unit A1-A3 A4 A5 B C1 C2 C3 C4 D
CR kg 0.00E+00 0.00E+00 1.53E-01 0 0.00E+00 0.00E+00 0.00E+00 0 0.00E+00
MR kg 3.44E-03 0.00E+00 1.09E+00 0 0.00E+00 0.00E+00 0.00E+00 0 8.50E+01
MER kg 0.00E+00 0.00E+00 3.76E-01 0 0.00E+00 0.00E+00 2.55E-03 0 0.00E+00
EEE MJ -1.54E-01 0.00E+00 -1.87E-01 0 0.00E+00 0.00E+00 1.40E+00 0 0.00E+00
ETE MJ -1.51E+02 0.00E+00 -4.81E-02 0 0.00E+00 0.00E+00 3.59E-01 0 0.00E+00
CR Components for reuse; MR Materials for recycling; MER Materials for energy recovery; EEE Exported
electric energy; ETE Exported thermal energy
Reading example: 9,0 E-03 = 9,0*10-3 = 0,009
EPD for the best environmental decision 11
Information describing the biogenic carbon content at the factory gate
Biogenic carbon content Unit Value
Biogenic carbon content in product kg C 0
Biogenic carbon content in the accompanying packaging kg C 0.0048
44/12 is the ratio between the molecular mass of CO2 and C molecules
Additional Norwegian requirements
Greenhouse gas emission from the use of electricity in the manufacturing phase
National production mix from import, low voltage (production of transmission lines, in addition
to direct emissions and losses in grid) of applied electricity for the manufacturing process (A3).
National electricity grid Unit Value
Denmark (residual fuel mix, Carbon Footprint, 2022) kg CO2 -eq/kWh 0.428
Additional environmental impact indicators required in NPCR Part A for construction
products
In order to increase the transparency of biogenic carbon contribution to climate impact, the
indicator for GWP has been sub-divided into the following:
GWP-IOBC Climate impacts calculated according to the principle of instantaneous oxidation
GWP-BC Climate impacts from the net uptake and emission of biogenic carbon from each
module.
In addition, EP-freshwater shall also declared as PO4 eq.
Indicator Unit A1 A2 A3 A1-A3
EP-freshwater* kg PO4 eq. 9.13E-03 1.63E-02 1.10E-03 2.65E-02
GWP-IOBC kg CO2 eq. 5.59E+00 5.62E+00 9.62E+00 2.08E+01
GWP-BC kg CO2 eq. 6.22E-02 4.81E-03 -4.89E-02 1.81E-02
GWP kg CO2 eq. 5.66E+00 5.63E+00 9.57E+00 2.09E+01
EP-freshwater* Eutrophication potential, fraction of nutrients reaching freshwater end compartment.
Declared as PO4 eq. GWP-IOBC Global warming potential calculated according to the principle of
instantaneous oxidation. GWP-BC Global warming potential from net uptake and emissions of biogenic
carbon from the materials in each module. GWP Global warming potential
EPD for the best environmental decision 12
Hazardous substances
The declaration is based upon reference to threshold values and/or test results and/or material
safety data sheets provided to EPD verifiers. Documentation available upon request to EPD
owner.
 The product contains no substances given by the REACH Candidate list or the
Norwegian priority list.
□ The product contains substances given by the REACH Candidate list or the Norwegian
priority list that are less than 0,1 % by weight.
□ The product contain dangerous substances, more then 0,1% by weight, given by the
REACH Candidate List or the Norwegian Priority list, see table.
□ The product contains no substances given by the REACH Candidate list or the
Norwegian priority list. The product is classified as hazardous waste (Avfallsforskiften,
Annex III), see table.
Indoor environment
The product meets the requirements for low emissions.
Carbon footprint
Carbon footprint has not been worked out for the product.
Bibliography
Calculla Chemical bond energies https://calculla.com/bond_energy, retrieved
2022-04-20
EPD PCR 2019 General Programme Instructions for the Norwegian EPD Foundation,
version 5
Gas consumption https://www.calculat.org/en/energy-fuel/gas-consumption.html,
retrieved 2022-02-14
Google Maps https://www.google.co.uk/maps, retrieved 2022-02-14
ISO 14025:2006 International Standard ISO 14025:2006 – Environmental labels and
declarations — Type III environmental declarations — Principles and
procedures
ISO 14040:2006 International Standard ISO 14040: Environmental Management – Life
cycle assessment – Principles and framework. Second edition 2006-07-
01.
ISO 14044:2006 International Standard ISO 14044: Environmental Management – Life
cycle assessment – Requirements and Guidelines.
EPD for the best environmental decision 13
ISO 15804:A2 2019 International Standard ISO 15804:2021 + A2: Sustainability of
construction works – Environmental product declarations – Core rules
for the product category of construction products
ISO 21930: 2007 International Standard ISO 21930:2007 Sustainability in building
construction – Environmental declaration of building products
Sea distances www.sea-distances.org, retrieved 2022-02-14
Statistics Denmark www.dst.dk/en, retrieved 2022-02-14
Program Operator
The Norwegian EPD Foundation tlf +47 23 08 80 00
Post Box 5250 Majorstuen, 0303 Oslo e-post: post@epd-norge.no
Norway web www.epd-norge.no
Publisher
The Norwegian EPD Foundation tlf +47 23 08 80 00
Post Box 5250 Majorstuen, 0303 Oslo e-post: post@epd-norge.no
Norway web www.epd-norge.no
Owner of the declaration
Nordisk Perlite ApS tlf +45 48 14 07 22
Hammersholt Erhvervspark 1-5 e-post: nordisk@perlite.dk
DK-3400 Hillerød, Denmark web www.nordiskperlite.com
Author of the life cycle assessment
Amy Stockwell tlf +44 7746 175762
Eando AB, Tåstrupsgatan 2, e-post: Amy.Stockwell@eando.se
SE-262 63 Ängelholm Sweden web www.eando.se
EPD for the best environmental decision 14
EPD for the best
environmental
decision
The Norwegian EPD foundation
www.epd-norge.no
EPD for the best environmental decision 15
