Environmental product declaration
in accordance with ISO 14025 and EN 15804+A2
Harmonie "Massiv" interior door without glass
Owner of the declaration: Program operator:
Harmonie Norge AS The Norwegian EPD Foundation
Product: Declaration number:
Harmonie "Massiv" interior door without glass
Registration number:
Declared unit:
1 pcs Issue date:
This declaration is based on Product Category Rules: Valid to:
CEN Standard EN 15804:2012+A2:2019 serves as core
EPD Software:
PCR
The Norwegian EPD Foundation LCA.no EPD generator ID: 169216
NPCR 014:2019 Part B for Windows and doors
1 / 12
General information
Product Owner of the declaration:
Harmonie "Massiv" interior door without glass Harmonie Norge AS
Contact person: Paul Roman
Phone: +47 94 98 04 80
e-mail: paul@harmonie.no
Program operator: Manufacturer:
Post Box 5250 Majorstuen, 0303 Oslo, Norway Harmonie Norge AS
The Norwegian EPD Foundation Borgeskogen 36
Phone: +47 23 08 80 00 3160 Stokke, Norway
web: post@epd-norge.no
Declaration number: Place of production:
Harmonie prod. Romania
, Romania
This declaration is based on Product Category Rules: Management system:
CEN Standard EN 15804:2012+A2:2019 serves as core PCR
NPCR 014:2019 Part B for Windows and doors
Statement of liability: Organisation no:
The owner of the declaration shall be liable for the underlying 912591743
information and evidence. EPD Norway shall not be liable with respect
to manufacturer information, life cycle assessment data and
evidences.​
Declared unit: Issue date:
1 pcs Harmonie "Massiv" interior door without glass
Declared unit with option: Valid to:
A1-A3,A4,A5,B2,B4,C1,C2,C3,C4,D
Year of study:
2022
Functional unit: Comparability:
Painted "Massiv" interior door without glass, dimension 1230 mm x EPD of construction products may not be comparable if they not
2180 mm (reference door based on EN 14351-1), and expected comply with EN 15804 and seen in a building context.
service life of 10 years.
General information on verification of EPD from EPD tools: Development and verification of EPD:
Independent verification of data, other environmental information The declaration is created using EPD tool lca.tools ver EPD2022.03,
and the declaration according to ISO 14025:2010, § 8.1.3 and § 8.1.4. developed by LCA.no. The EPD tool is integrated in the company's
Verification of each EPD is made according to EPD-Norway’s management system, and has been approved by EPD Norway.
guidelines for verification and approval requiring that tools are i)
integrated into the company's environmental management system, ii) Developer of EPD: Solmaz Atarodi
the procedures for use of the EPD tool are approved by EPD-Norway,
Reviewer of company-specific input data and EPD:​ Paul Roman
and iii) the process is reviewed annually by an independent third
party verifier. See Appendix G of EPD-Norway's General Programme
Instructions for further information on EPD tools
Verification of EPD tool: Approved:
Independent third party verification of the EPD tool, background data
and test-EPD in accordance with EPDNorway's procedures and
guidelines for verification and approval of EPD tools. Håkon Hauan, CEO EPD-Norge
Third party verifier:
Gaylord K. Booto, Norwegian Institute for Air Research (NILU)
(no signature required)
2 / 12
Product
Product description:
Harmonie "Massiv" interior door used on walls in residential and non-residential constructions.
Product specification
This EPD applies to an interior door with painted surfaces. The door size is 1230 mm x 2180 mm.
Materials kg %
Glue for wood 0,22 0,59
Metal - Steel 0,23 0,61
Paint, water-based 0,75 2,00
Wood - Fibreboard 28,63 76,20
Wood - Laminated wood 7,74 20,60
Total 37,57
Packaging kg %
Packaging - Cardboard 0,26 18,87
Packaging - Plastic 0,21 15,24
Packaging - Wood 0,91 65,89
Total incl. packaging 38,94
Technical data:
Interior door with HDF panel, HDF/Timber rails and stiles, one lock and two hinges. The thickness of doorleaf is 40mm. The total weight of the
product is 37.57 kg and the packaging avaerage weight is 1.38 kg. Area of function unit is 2.68 m². The product is available in the majority of NCS
S / RAL color palettes.
Market:
Scandinavian countries, but scenarios beyond cradle-to-gate are based on the situation in the Norwegian market.
Reference service life, product
10 years
Reference service life, building or construction works
60 years.
LCA: Calculation rules
Declared unit:
1 pcs Harmonie "Massiv" interior door without glass
Cut-off criteria:
All major raw materials and all the essential energy is included. The production processes for raw materials and energy flows with very small
amounts (less than 1%) are not included. These cut-off criteria do not​ apply for hazardous materials and substances.
Allocation:
The allocation is made in accordance with the provisions of EN 15804. Effects of primary production of recycled materials is allocated to the main
product in which the material was used. The recycling process and transportation of the material is allocated to this analysis. The PCR specific
background data follow the allocation rules in the Ecoinvent v3.7.1 Cut-off database version. The allocation of water, energy and waste flows
within the production facilities for windows and doors follows unit-based allocation adjusted with a point system to different product groups or
products. This score system is regulated by a factor which increases with the resource intensity of each product. The unit-based allocation is
adjusted by the weight of the product, excluding the weight of glass.
Data quality:
Specific data for the product composition are provided by the manufacturer. The data represent the production of the declared product and were
collected for EPD development in the year of study. Background data is based on EPDs according to EN 15804 and different LCA databases. The
data quality of the raw materials in A1 is presented in the table below.
Materials Source Data quality Year
Glue for wood ecoinvent 3.6 Database 2019
Metal - Steel ecoinvent 3.6 Database 2019
Packaging - Cardboard ecoinvent 3.6 Database 2019
Packaging - Plastic ecoinvent 3.6 Database 2019
Packaging - Wood ecoinvent 3.6 Database 2019
Wood - Fibreboard ecoinvent 3.6 Database 2019
Wood - Laminated wood ecoinvent 3.6 Database 2019
Paint, water-based ecoinvent 3.7.1 Database 2020
3 / 12
System boundaries (X=included, MND=module not declared, MNR=module not relevant)
Construction Beyond the system
Product stage Use stage End of life stage
installation stage boundaries
A1 A2 A3 A4 A5 B1 B2 B3 B4 B5 B6 B7 C1 C2 C3 C4 D
X X X X X MND X MND X MND MND MND X X X X X
System boundary:
According to the standard NS-EN 15804:2012+A2:2019, NPCR PART A (construction products and services), and NPCR 014 (Part B for windows
and doors), the system boundary is cradle to grave and module D.
Additional technical information:
For the products with different sizes from the declared unit, the environmental impacts must be converted by using a conversion factor. The
Norwegian EPD Foundation has published instructions on how to interpret EPDs for Windows on its website (www.epdnorge.no) where different
calculation methods have been stated. (Document: Bruksanvisninger i hvordan tolke EPD'er - Vinduer).
waR slairetam tropsnarT gnirutcafunaM tropsnarT ylbmessA e​sU ecnanetniaM riapeR tnemecalpeR tnemhsibrufeR lanoitarepO ygrene esu lanoitarepO esu retaw -eD noitcurtsnoc noitilomed tropsnarT etsaW gnissecorp lasopsiD -yrevoceR-esueR laitnetop-gnilcyceR
4 / 12
LCA: Scenarios and additional technical information
The following information describe the scenarios in the different modules of the EPD.
A4- Transport
Based on information from the manufacturer, the transportation scenario for the final packed product from the manufacturer to the construction
site is as the following: from the factory in Romania to the warehouse in Stokke, Norway: 452 km by Euro 6- medium truck, 1376 km by train, 99
km by boat, and 568 km by Euro 6- medium truck.
The average transportation distance from the warehouse to the installation site is assumed 50 km by medium truck.
A5- Assembly
According to the report from EPD-Norge Harmonising the documentation of scenarios beyond cradle to gate, EN 15804 there is no loss on-site
during construction activities. Since painting and surface treatment are done before installation, installation materials are negligible and not
included in this assessment. Energy consumption during installation can be varied depending on the floor, type of building, and several other
unknown parameters, and therefore ignored in the calculation. So, the installation module includes waste treatment of packaging waste.
The contribution from auxiliary materials used for installation, e.g., fixings, sealants, and insulation materials, is commonly considered to be within
the cut-off criteria (6.3.4.3 Construction stage, NS-EN 17213:2020).
B1- Use
Use of the installed product in terms of any emissions to the environment (not covered by B2-B7). Module not declared.
B2- Maintenance
The maintenance scenario includes cleaning and painting. Cleaning is performed two times washing per year for doors without glass. It is
calculated with 45 ml of detergent and 4.5 liters of water each year during RSL of the building.
Doors are assumed to be painted 1 time during their lifetime. It is assumed that 5 gr of lubricating oil is used every year for fittings and moving
parts.
B3- Repair
No repair is assumed during the product’s lifetime. Module not declared.
B4- Replacement
The door has an RSL (Reference Service Life) of 10 years. If the lifetime of the building is assumed 60 years, a five-time replacement.
B5- Refurbishment
There is no need for refurbishment during the product’s lifetime. Module not declared.
B6 and B7
Module not declared.
C1- Deconstruction demolition
In the C module, the end-of-life scenario is assumed that the door is demounted during the deconstruction process and no separate energy from
a machine is required for this process.
C2-Transport
The entire door is transported to a municipal waste collection and sorting station, and the average transport distance from the demolition place to
the station is assumed to be 85 km.
C3- Waste processing
Based on Table 1 in NPCR 014 Part B- Windows and Doors, the door is assumed as mixed waste and sent to municipal incineration with energy
recovery.
C4- Disposal
The ashes from municipal incineration, that are not separated for recycling goals, are transferred to landfilling.
D- Benefits and loads beyond the system boundaries
The combustible materials (plastic and timber) are considered as energy recovered materials. Energy recovery from incineration is assumed with
the process efficiency rate of the power station above 60 %.
The metals are separated from the bottom ashes and recycled. Since there is no data on the share recycled, the Ecoinvent database is employed
(B.3, NS-EN 17213:2020) Here the assumption is that recovered metals can be substituted by the primary metals used (6.4.3.3, EN 15804).
Capacity utilisation Value
Transport from production place to user (A4) Distance (km) Fuel/Energy Consumption Unit
(incl. return) % (Liter/tonne)
Ship, Ferry, Sea (km) 50,0 % 99 0,034 l/tkm 3,37
Train, freight (kgkm) 0,0 % 1376 0,000 0 0,00
Truck, 16-32 tonnes, EURO 6 (km) - Europe 36,7 % 568 0,043 l/tkm 24,42
Truck, 16-32 tonnes, EURO 6 (km) - Europe 36,7 % 50 0,043 l/tkm 2,15
Truck, 16-32 tonnes, EURO 6 (km) - Europe 36,7 % 452 0,043 l/tkm 19,44
5 / 12
Assembly (A5) Unit Value
Waste, packaging, cardboard, to average
kg 0,26
treatment (kg)
Waste, packaging, pallet, wooden pallet, single
kg 0,91
use, average treatment (kg)
Waste, packaging, plastic film (LDPE), to average
kg 0,22
treatment (kg)
Maintenance (B2) Unit Value
Lubricant (kg) kg/DU 0,30
Paint wastage, 40% water, wet mass (kg) kg 0,06
Paint, 40% water, wet mass (kg) inkl. 5% waste kg/DU 1,20
Soap water, 5% solution with household detergent
kg/DU 1,82
(kg)
Waste paint, 40% water, wet mass, incineration in
kg 0,06
Norway (kg)
Wastewater, average treatment (m3) m3 0,18
Water, tap water (kg) kg/DU 180,00
Replacement (B4) Unit Value
Replace product (pcs) Units/DU 5,00
Waste treatment of replaced product (pcs) Units 5,00
Capacity utilisation Value
Transport to waste processing (C2) Distance (km) Fuel/Energy Consumption Unit
(incl. return) % (Liter/tonne)
Truck, unspecified (km) - Europe 48,7 % 85 0,051 l/tkm 4,34
Waste processing (C3) Unit Value
Materials to recycling (kg) kg 0,48
Waste treatment per kg Cardboard and paper,
kg 0,96
incineration with fly ash extraction (kg)
Waste treatment per kg Paint, hazardous waste
kg 1,43
incineration (kg)
Waste treatment per kg Polyurethane (PU),
kg 0,21
incineration (kg)
Waste treatment per kg Wood, incineration with
kg 52,76
fly ash extraction (kg)
Disposal (C4) Unit Value
Landfilling of ashes from incineration of
Cardboard and paper, process per kg ashes and kg 0,02
residues (kg)
Landfilling of ashes from incineration of Paint,
hazardous waste incineration, process of ashes kg 0,04
and residues (kg)
Landfilling of ashes from incineration of
Polyurethane (PU), process per kg ashes and kg 0,02
residues - C4 (kg)
Landfilling of ashes from incineration of Wood,
kg 0,61
process per kg ashes and residues (kg)
Waste, cardboard and paper, to landfill (kg) kg 0,05
Waste, glue, to landfill (kg) kg 0,01
Waste, paint, to landfill (kg) - C4 kg 0,04
Waste, scrap steel, to landfill (kg) kg 0,03
Waste, wood, untreated, to landfill (kg) kg 2,54
Benefits and loads beyond the system
Unit Value
boundaries (D)
Substitution of electricity, in Norway (MJ) MJ 38,31
Substitution of primary steel with net scrap (kg) kg 0,48
Substitution of thermal energy, district heating, in
MJ 579,54
Norway (MJ)
6 / 12
LCA: Results
The LCA results are presented below for the declared unit defined on page 2 of the EPD document.
Environmental impact
Indicator Unit A1-A3 A4 A5 B2 B4 C1 C2 C3 C4 D
GWP-total
kg CO2 -
-1,24E+01 9,77E+00 1,86E+00 7,39E+00 5,09E+02 0 4,36E-01 1,02E+02 3,85E-01 -4,01E+00
eq
GWP-fossil
kg CO2 -
4,90E+01 9,76E+00 4,61E-02 6,09E+00 3,26E+02 0 4,36E-01 5,90E+00 6,89E-02 -3,88E+00
eq
GWP-biogenic
kg CO2 -
-6,28E+01 7,75E-03 1,82E+00 1,12E-01 1,76E+02 0 1,87E-04 9,58E+01 3,16E-01 -7,23E-03
eq
GWP-luluc
kg CO2 -
1,43E+00 6,15E-03 8,99E-06 1,18E+00 7,19E+00 0 1,54E-04 5,46E-04 1,17E-05 -1,16E-01
eq
kg
ODP CFC11 - 3,52E-06 2,00E-06 5,84E-09 1,08E-06 2,99E-05 0 9,93E-08 3,40E-07 1,22E-08 -2,45E-01
eq
mol H+
AP 3,59E-01 5,64E-02 2,38E-04 6,21E-02 2,16E+00 0 2,48E-03 1,30E-02 3,41E-04 -3,03E-02
-eq
EP-FreshWater kg P -eq 6,85E-03 1,26E-04 3,63E-07 1,90E-03 3,50E-02 0 3,58E-06 1,86E-05 9,16E-07 -3,31E-04
EP-Marine kg N -eq 1,43E-01 1,62E-02 1,11E-04 1,48E-02 8,26E-01 0 8,88E-04 5,08E-03 2,84E-04 -9,59E-03
mol N -
EP-Terrestial 5,86E-01 1,79E-01 1,05E-03 7,81E-02 4,16E+00 0 9,78E-03 5,44E-02 1,29E-03 -1,03E-01
eq
kg
POCP NMVOC 2,19E-01 5,31E-02 2,78E-04 3,21E-02 1,45E+00 0 2,80E-03 1,42E-02 4,51E-04 -2,96E-02
-eq
ADP- kg Sb -
1,62E-03 2,11E-04 5,91E-07 7,87E-05 9,25E-03 0 1,13E-05 6,79E-06 4,03E-07 -4,24E-05
minerals&metals1 eq
ADP-fossil1 MJ 6,97E+02 1,41E+02 4,18E-01 1,03E+02 4,35E+03 0 6,69E+00 2,31E+01 9,51E-01 -5,24E+01
WDP1 m3 9,32E+03 1,43E+02 7,71E-01 8,52E+01 4,78E+04 0 6,34E+00 8,98E+01 8,65E+00 -5,71E+02
GWP-total = Global Warming Potential total; GWP-fossil = Global Warming Potential fossil fuels; GWP-biogenic = Global Warming Potential biogenic; GWP-luluc =
Global Warming Potential land use and land use change; ODP = Depletion potential of the stratospheric ozone layer; AP = Acidification potential, Accumulated
Exceedance; EP-freshwater = Eutrophication potential, fraction of nutrients reaching freshwater end compartment: EP-marine = Eutrophication potential, fraction of
nutrients reaching marine end compartment; EP-terrestrial = Eutrophication potential, Accumulated Exceedance; POCP = Formation potential of tropospheric ozone;
ADP-minerals&metals = Abiotic depletion potential for non-fossil resources; ADP-fossil = Abiotic depletion for fossil resources potential; WDP = Water (user)
deprivation potential, deprivation-weighted water consumption
"Reading example: 9,0 E-03 = 9,0*10-3 = 0,009"
*INA Indicator Not Assessed
1. The results of this environmental impact indicator shall be used with care as the uncertainties on these results are high or as there is limited experienced with the
indicator
Remarks to environmental impacts
7 / 12
Additional environmental impact indicators
Indicator Unit A1-A3 A4 A5 B2 B4 C1 C2 C3 C4 D
PM Disease incidence 4,36E-06 6,43E-07 3,08E-09 4,32E-07 2,62E-05 0 3,97E-08 1,86E-07 5,77E-09 -1,72E-06
IRP2 kgBq U235 -eq 3,91E+00 6,24E-01 1,62E-03 3,62E-01 2,33E+01 0 2,92E-02 9,48E-02 4,54E-03 -3,05E-01
ETP-fw1 CTUe 1,21E+03 1,19E+02 4,74E-01 2,23E+02 6,85E+03 0 5,00E+00 3,33E+01 1,14E+00 -2,90E+02
HTP-c1 CTUh 7,84E-08 0,00E+00 4,00E-11 1,00E-08 4,52E-07 0 0,00E+00 1,20E-08 5,20E-11 -7,30E-09
HTP-nc1 CTUh 8,13E-07 1,41E-07 1,91E-09 1,43E-07 5,39E-06 0 6,62E-09 1,14E-07 1,66E-09 -1,96E-07
SQP1 dimensionless 6,34E+03 9,60E+01 3,26E-01 1,10E+02 3,23E+04 0 5,72E+00 9,95E+00 3,63E+00 -3,22E+02
PM = Particulate Matter emissions; IRP = Ionizing radiation – human health; ETP-fw = Eco toxicity – freshwater; HTP-c = Human toxicity – cancer effects; HTP-nc =
Human toxicity – non cancer effects; SQP = Potential Soil Quality Index (dimensionless)
"Reading example: 9,0 E-03 = 9,0*10-3 = 0,009"
*INA Indicator Not Assessed
1. The results of this environmental impact indicator shall be used with care as the uncertainties on these results are high or as there is limited experienced with the
indicator
2. This impact category deals mainly with the eventual impact of low dose ionizing radiation on human health of the nuclear fuel cycle. It does not consider effects due
to possible nuclear accidents, occupational exposure nor due to radioactive waste disposal in underground facilities. Potential ionizing radiation from the soil, from
radon and from some construction materials is also not measured by this indicator.
8 / 12
Resource use
Indicator Unit A1-A3 A4 A5 B2 B4 C1 C2 C3 C4 D
PERE MJ 7,39E+02 3,46E+00 8,68E-03 1,64E+01 3,74E+03 0 9,59E-02 4,14E+00 4,80E-02 -2,97E+02
PERM MJ 4,04E+02 0,00E+00 -1,47E+01 0,00E+00 -1,02E+03 0 0,00E+00 -5,93E+02 0,00E+00 0,00E+00
PERT MJ 1,14E+03 3,46E+00 -1,47E+01 1,64E+01 2,72E+03 0 9,59E-02 -5,89E+02 4,80E-02 -2,97E+02
PENRE MJ 6,74E+02 1,41E+02 4,18E-01 9,72E+01 4,23E+03 0 6,69E+00 2,31E+01 9,51E-01 -5,24E+01
PENRM MJ 2,67E+01 0,00E+00 -9,34E+00 7,30E+00 -3,86E+01 0 0,00E+00 -2,51E+01 0,00E+00 0,00E+00
PENRT MJ 7,01E+02 1,41E+02 -8,93E+00 1,05E+02 4,20E+03 0 6,69E+00 -2,01E+00 9,51E-01 -5,24E+01
SM kg 2,40E-01 0,00E+00 0,00E+00 0,00E+00 1,20E+00 0 0,00E+00 0,00E+00 2,88E-04 0,00E+00
RSF MJ 6,42E+00 8,31E-02 2,52E-04 3,09E-02 3,30E+01 0 3,41E-03 8,64E-02 1,09E-03 -3,31E-02
NRSF MJ 4,98E-01 4,02E-01 2,22E-03 8,55E-03 5,67E+00 0 1,20E-02 0,00E+00 2,19E-01 -1,70E+01
FW m3 6,33E-01 2,45E-02 2,75E-04 1,30E-01 3,38E+00 0 7,57E-04 1,59E-02 1,07E-03 -3,59E-01
PERE = Use of renewable primary energy excluding renewable primary energy resources used as raw materials; PERM = Use of renewable primary energy resources used
as raw materials; PERT = Total use of renewable primary energy resources; PENRE = Use of non renewable primary energy excluding non-renewable primary energy
resources used as raw materials; PENRM = Use of non renewable primary energy resources used as raw materials; PENRT = Total use of non renewable primary energy
resources; SM = Use of secondary materials; RSF = Use of renewable secondary fuels; NRSF = Use of non-renewable secondary fuels; FW = Net use of fresh water
"Reading example: 9,0 E-03 = 9,0*10-3 = 0,009"
*INA Indicator Not Assessed
9 / 12
End of life - Waste
Indicator Unit A1-A3 A4 A5 B2 B4 C1 C2 C3 C4 D
HWD kg 3,80E-01 1,41E-02 0,00E+00 4,98E-02 4,33E+00 0 3,61E-04 0,00E+00 4,71E-01 -4,97E-03
NHWD kg 1,08E+01 5,49E+00 1,39E+00 3,88E+00 1,05E+02 0 4,14E-01 0,00E+00 2,95E+00 -1,35E+00
RWD kg 3,34E-03 9,23E-04 0,00E+00 4,74E-04 2,16E-02 0 4,55E-05 0,00E+00 5,66E-06 -2,50E-04
HWD = Hazardous waste disposed; NHWD = Non-hazardous waste disposed; RWD = Radioactive waste disposed
"Reading example: 9,0 E-03 = 9,0*10-3 = 0,009"
*INA Indicator Not Assessed
End of life - Output flow
Indicator Unit A1-A3 A4 A5 B2 B4 C1 C2 C3 C4 D
CRU kg 0,00E+00 0,00E+00 0,00E+00 0,00E+00 0,00E+00 0 0,00E+00 0,00E+00 0,00E+00 0,00E+00
MFR kg 1,11E+00 0,00E+00 3,54E-01 0,00E+00 9,70E+00 0 0,00E+00 4,75E-01 2,33E-04 0,00E+00
MER kg 2,69E-01 0,00E+00 9,19E-01 0,00E+00 2,76E+02 0 0,00E+00 5,39E+01 5,19E-06 0,00E+00
EEE MJ 2,25E-01 0,00E+00 6,41E-01 3,54E-02 1,93E+02 0 0,00E+00 3,78E+01 3,67E-04 0,00E+00
EET MJ 3,41E+00 0,00E+00 9,70E+00 2,46E-01 2,92E+03 0 0,00E+00 5,71E+02 5,56E-03 0,00E+00
CRU = Components for re-use; MFR = Materials for recycling; MER = Materials for energy recovery; EEE = Exported energy electrical; EET = Exported energy thermal
"Reading example: 9,0 E-03 = 9,0*10-3 = 0,009"
*INA Indicator Not Assessed
Biogenic Carbon Content
Indicator Unit At the factory gate
Biogenic carbon content in product kg C 1,68E+01
Biogenic carbon content in accompanying packaging kg C 4,96E-01
Note: 1 kg biogenic carbon is equivalent to 44/12 kg CO2
10 / 12
Additional requirements
Greenhouse gas emissions from the use of electricity in the manufacturing phase
National production mix from import, low voltage (production of transmission lines, in addition to direct emissions and losses in grid) of applied
electricity for the manufacturing process (A3).
Electricity mix Data source Amount Unit
Electricity, Romania (kWh) ecoinvent 3.6 465,15 g CO2-eq/kWh
Electricity, Norway (kWh) ecoinvent 3.6 24,33 g CO2-eq/kWh
Dangerous substances
The product contains no substances given by the REACH Candidate list.
Indoor environment
Additional Environmental Information
Additional environmental impact indicators required in NPCR Part A for construction products
Indicator Unit A1-A3 A4 A5 B2 B4 C1 C2 C3 C4 D
GWPIOBC kg CO2 -eq 5,09E+01 9,77E+00 4,53E-02 7,92E+00 3,21E+02 0 4,36E-01 2,76E+00 2,01E-01 -4,21E+00
GWP-IOBC: Global warming potential calculated according to the principle of instantaneous oxidation. In order to increase the transparency of biogenic carbon​
contribution to climate impact, the indicator GWP-IOBC is required as it declares climate impacts calculated according to the principle of instantaneous oxidation.​
GWP-IOBC is also referred to as GWP-GHG in context to Swedish public procurement legislation.
11 / 12
Bibliography
ISO 14025:2010 Environmental labels and declarations - Type III environmental declarations - Principles and procedures.
ISO 14044:2006 Environmental management - Life cycle assessment - Requirements and guidelines.
EN 15804:2012+A2:2019 Environmental product declaration - Core rules for the product category of construction products.
ISO 21930:2017 Sustainability in buildings and civil engineering works - Core rules for environmental product declarations of construction
products.
ecoinvent v3, Allocation, cut-off by classification, Swiss Centre of Life Cycle Inventories.
Iversen et al., (2021) eEPD v2021.09 Background information for EPD generator tool system verification, LCA.no Report number: 07.21
Iversen et al., (2022) EPD generator for EPD generator for NPCR 014
Part B for Windows and doors, Background information for EPD generator application and LCA data, LCA.no report number: 17.22
NPCR Part A: Construction products and services. Ver. 2.0. April 2021, EPD-Norge.
NPCR 014 Part B for Windows and doors, Ver. 4.0, 20.09.2021, EPD Norway.
Program operator and publisher Phone: +47 23 08 80 00
The Norwegian EPD Foundation e-mail: post@epd-norge.no
Post Box 5250 Majorstuen, 0303 Oslo, Norway web: www.epd-norge.no
Owner of the declaration: Phone: +47 94 98 04 80
Harmonie Norge AS e-mail: paul@harmonie.no
Borgeskogen 36, 3160 Stokke web: https://harmonie.no/
Author of the Life Cycle Assessment Phone: +47 916 50 916
LCA.no AS e-mail: post@lca.no
Dokka 6B, 1671 web: www.lca.no
Developer of EPD generator Phone: +47 916 50 916
LCA.no AS e-mail: post@lca.no
Dokka 6B,1671 Kråkerøy web: www.lca.no
ECO Platform web: www.eco-platform.org
ECO Portal web: ECO Portal
12 / 12
