ver1 2015
ENVIRONMENTAL PRODUCT DECLARATION
in accordance with ISO 14025, ISO 21930 and EN 15804
Owner of the declaration: Flokk AS
Program operator: The Norwegian EPD Foundation
Publisher: The Norwegian EPD Foundation
Declaration number: NEPD-3468-2072-EN
Registration number: NEPD-3468-2072-EN
ECO Platform reference number: -
Issue date: 26.04.2022
Valid to: 26.04.2027
giroflex 40
Flokk AS
www.epd-norge.no
NEPD-3468-2072-EN giroflex 40
1 / 8
General information
Product: Owner of the declaration:
giroflex 40
Flokk AS
Contact person: Atle Thiis-Messel
Phone: 0047 98 25 68 30
e-mail: atle.messel@flokk.com
Program operator: Manufacturer:
Flokk AS
The Norwegian EPD Foundation
Drammensveien 145, 0277 Oslo
Pb. 5250 Majorstuen, 0303 Oslo
Norway
Phone: +47 23 08 80 00
e-mail: post@epd-norge.no
Declaration number: Place of production:
Flokk - Turek
NEPD-3468-2072-EN ul. Górnicza 8 62-700 Turek
Poland
ECO Platform reference number: Management system:
ISO 14001, ISO 9001, ISO 50001(Norway, Sweden)
This declaration is based on Product Category Rules: Organisation no:
No 928 902 749
CEN Standard EN 15804:2012+A1:2013 serves as core PCR
NPCR 026:2018 Part B for furniture
Statement of liability: Issue date: 26.04.2022
The owner of the declaration shall be liable for the underlying information and
evidence. EPD Norway shall not be liable with respect to manufacturer Valid to: 26.04.2027
information, life cycle assessment data and evidences.
Declared unit: Year of study:
1 Pcs giroflex 40 2022
Declared unit with option: Comparability:
A1,A2,A3,A4 EPDs from programmes other than the Norwegian EPD Foundation may not be
comparable
Functional unit: Development and verification of EPD:
giroflex 40 - 1 pc The declaration has been developed and verified using EPD tool lca.tools
ver EPD2020.11, developed by LCA.no AS. The EPD tool is integrated into
the company's environmental management system, and has been
approved by EPD-Norway
General information on verification of EPD from EPD tools:
Independent verification of data, other environmental information and Developer of EPD:
the declaration according to ISO 14025:2010, § 8.1.3 and § 8.1.4. Individual
third party verification of each EPD is not required when the EPD tool is i) Damian Bakowski
integrated into the company's environmental management system, ii) the
procedures for use of the EPD tool are approved by EPDNorway, and iii) Reviewer of company-specific input data and EPD:
the proccess is reviewed annualy. See Appendix G of EPD-Norway's
General Programme Instructions for further information on EPD tools. Arleta Derdziak
Verification of EPD tool: Approved:
Independent third party verification of the EPD tool, background data
Sign
and test-EPD in accordance with EPDNorway's procedures and guidelines
for verification and approval of EPD tools.
Erik Svanes, Norsus AS
(no signature required) Håkon Hauan, CEO EPD-Norge
Key environmental indicators Unit Cradle to gate A1 - A3
Global warming kg CO2 eqv 80,16
Total energy use MJ 1108,48
Amount of recycled materials % 32.17
NEPD-3468-2072-EN giroflex 40
2 / 8
Product
Market: Technical data:
worldwide
Seat height loaded: 375-515 mm
Product description:
Total height (without headrest): 995-1135 mm
The giroflex 40 is an elegant, energizing contribution to
Backrest height above seat: 620 mm
a work environment, with its health-focused purpose designed
with a harmonic approach.
Seat width: 510 mm
The holistic and timeless design of giroflex 40, is a synergetic
Backrest width: 445 mm
combination of the forwarded circular Giroflex-DNA and discreetly
placed functional details in its platform and seat, brought to you with
Total width (5 arm base): 660 mm (diameter 720 mm)
outstanding quality that enhance the bloodstream in your body.
Seat depth: 420-480 mm
The giroflex 40 offers a large variety of functions already included in
the standard version and offers an essential range of options and
Armrest height above seat: 170-260 mm
variants for a fast and easy decisionmaking.
Product specification Seat inclination angle: 0°-3°
Please look in additional technical information, page 8.
Reference service life, product
5 years
Reference service life, building
Recycled share in Recycled share in
Materials kg %
material (kg) material (%)
Metal - Aluminium 4,88 23,22 4,76 97,54
Metal - Steel 4,97 23,65 0,68 13,69
Textile - Polyester (PE) 0,35 1,68 0,19 54,55
Plastic - Polyurethane (PUR) 0,85 4,05 0,00 0,00
Plastic - Acrylonitrile butadiene styrene (ABS) 0,01 0,05 0,00 0,00
Plastic - Polypropylene (PP) 4,18 19,88 0,00 0,00
Plastic - Polyoxymethylene (POM) 0,17 0,79 0,00 0,00
Rubber, synthetic 0,02 0,10 0,00 0,00
Packaging - Plastic 0,24 1,14 0,00 0,00
Powder coating 0,01 0,06 0,00 0,00
Plastic - Nylon (PA) 1,34 6,36 0,00 0,00
Plastic - Polyamide with glass fibre (PAGF30) 0,49 2,32 0,00 0,00
Plastic - Polyester 0,01 0,05 0,00 0,00
Total: 17,50 5,63
LCA: Calculation rules
Declared unit: Allocation:
The allocation is made in accordance with the provisions of EN 15804. Effects
1 Pcs giroflex 40
of primary production of recycled materials is allocated to the main product
Cut-off criteria: in which the material was used. The recycling process and transportation of
the material is allocated to this analysis.
All major raw materials and all the essential energy is included. The
production processes for raw materials and energy flows with very small
amounts (less than 1%) are not included. These cut-off criteria do not
apply for hazardous materials and substances.
Data quality:
Specific data for the product composition are provided by the manufacturer. They represent the production of the declared product and were collected for
EPD development in the year of study. Background data is based on registered EPDs according to EN 15804, Ostfold Research databases, ecoinvent and other
LCA databases. The data quality of the raw materials in A1 is presented in the table below.
NEPD-3468-2072-EN giroflex 40
3 / 8
System boundary:
Additional technical information:
Mechanism Synchro Move
Giroflex office chairs offer synchro motion, resulting in a natural body movement as you recline in the chair. The more backward you recline the seat, the
more your upper body will open up. This movement is created by the synchro mechanism, which drives the motion of the seat and backrest individually,
at a ratio of approx. 1:2
Mesh back
Pronounced ergonomic design for optimal adaptation and support. The mesh fabric RUNNER from Camira guarantees optimal comfort and air circulation.
Lumbar support
Height adjustable.
Handles in black plastic, for height adjustment and activation/de-activation of lumbar support function.
Seat with dual-zone profile
The front part (approx. 1/3 of the seat surface) has a 7° forward tilt to relieve pressure on thighs for optimal blood circulation.
Seat-and back frame
Aluminium, polished or powder coated black 810.
Base
5-arm plastic, black 810.
Optional: 5-arm aluminium, polished or powder coated black 810.
Armrest 3D - optional
Height adjustable, with longitudinal and sidewardly slidable armpad.
Headrest - optional
Height adjustable, headrest support aluminium black 810.
Covered by the fabric of seat, when mounted in the fabric of seat.
Optional: mesh RUNNER or Leather NATURA.
Castors
Ø50 mm black, for hard or soft floors, braked unloaded.
Optional: Ø 65 mm black, for hard or soft floors, braked unloaded.
NEPD-3468-2072-EN giroflex 40
4 / 8
LCA: Scenarios and additional technical information
The following information describe the scenarios in the different modules of the EPD.
Transport from production place to user (A4)
Capacity utilisation Fuel/Energy
Type Type of vehicle Distance km Unit Value (l/t)
(incl. return) % consumption
Truck 38,8 % Truck, 16-32 tonnes, EURO 5 1000 0,044606 l/tkm 44,61
Railway l/tkm
Boat l/tkm
Other Transportation l/tkm
NEPD-3468-2072-EN giroflex 40
5 / 8
LCA: Results
The LCA results are presented below for the declared unit defined on page 2 of the EPD document.
System boundaries (X=included, MND=module not declared, MNR=module not relevant)
Construction Beyond the
Product stage installation User stage End of life stage . system
stage bondaries
A1 A2 A3 A4 A5 B1 B2 B3 B4 B5 B6 B7 C1 C2 C3 C4 . D
X X X X MND MND MND MND MND MND MND MND MND MND MND MND . MND
Environmental impact
Parameter Unit A1 A2 A3 A4
GWP kg CO 2 -eq 7,21E+01 1,94E+00 6,12E+00 2,85E+00
ODP kg CFC11 -eq 3,18E-06 3,73E-07 1,58E-07 5,25E-07
POCP kg C 2H 4-eq 2,00E-02 4,67E-04 1,39E-03 4,64E-04
AP kg SO 2 -eq 2,94E-01 1,15E-02 3,68E-02 9,08E-03
EP kg PO 3- -eq 4,89E-02 1,44E-03 4,47E-03 1,51E-03
4
ADPM kg Sb -eq 2,00E-03 3,81E-06 3,39E-07 8,68E-06
ADPE MJ 8,07E+02 2,99E+01 6,23E+01 4,29E+01
GWP Global warming potential; ODP Depletion potential of the stratospheric ozone layer; POCP Formation potential of tropospheric photochemical oxidants;
AP Acidification potential of land and water; EP Eutrophication potential; ADPM Abiotic depletion potential for non fossil resources; ADPE Abiotic depletion
potential for fossil resources
Reading example: 9,0 E-03 = 9,0*10-3 = 0,009
*INA Indicator Not Assessed
waR slairetam tropsnarT gnirutcafunaM tropsnarT ylbmessA esU ecnanetniaM riapeR tnemecalpeR tnemhsibrufeR lanoitarepO ygrene esu lanoitarepO esu
retaw
-eD noitcurtsnoc noitilomed tropsnarT etsaW gnissecorp lasopsiD -yrevoceR-esueR -gnilcyceR laitnetop
NEPD-3468-2072-EN giroflex 40
6 / 8
Resource use
Parameter Unit A1 A2 A3 A4
RPEE MJ 7,33E+01 5,65E-01 7,31E+00 6,25E-01
RPEM MJ 2,74E-01 0,00E+00 0,00E+00 0,00E+00
TPE MJ 7,36E+01 5,65E-01 7,31E+00 6,25E-01
NRPE MJ 9,31E+02 3,09E+01 6,58E+01 4,39E+01
NRPM MJ 2,63E+02 0,00E+00 0,00E+00 0,00E+00
TRPE MJ 1,19E+03 3,09E+01 6,58E+01 4,39E+01
SM kg 5,63E+00 0,00E+00 0,00E+00 0,00E+00
RSF MJ 0,00E+00 0,00E+00 0,00E+00 0,00E+00
NRSF MJ 0,00E+00 0,00E+00 0,00E+00 0,00E+00
W m3 5,88E-01 6,85E-03 3,28E-02 8,22E-03
RPEE Renewable primary energy resources used as energy carrier; RPEM Renewable primary energy resources used as raw materials; TPE Total use of renewable
primary energy resources; NRPE Non renewable primary energy resources used as energy carrier; NRPM Non renewable primary energy resources used as
materials; TRPE Total use of non renewable primary energy resources; SM Use of secondary materials; RSF Use of renewable secondary fuels; NRSF Use of non
renewable secondary fuels; W Use of net fresh water
Reading example: 9,0 E-03 = 9,0*10-3 = 0,009
*INA Indicator Not Assessed
End of life - Waste
Parameter Unit A1 A2 A3 A4
HW kg 3,91E-02 1,67E-05 3,14E-02 2,56E-05
NHW kg 3,40E+01 2,46E+00 2,28E+00 2,31E+00
RW kg INA* INA* INA* INA*
HW Hazardous waste disposed; NHW Non hazardous waste disposed; RW Radioactive waste disposed
Reading example: 9,0 E-03 = 9,0*10-3 = 0,009
*INA Indicator Not Assessed
End of life - Output flow
Parameter Unit A1 A2 A3 A4
CR kg 0,00E+00 0,00E+00 0,00E+00 0,00E+00
MR kg 0,00E+00 0,00E+00 7,67E-01 0,00E+00
MER kg 0,00E+00 0,00E+00 4,70E-03 0,00E+00
EEE MJ INA* INA* INA* INA*
ETE MJ INA* INA* INA* INA*
CR Components for reuse; MR Materials for recycling; MER Materials for energy recovery; EEE Exported electric energy; ETE Exported thermal energy
Reading example: 9,0 E-03 = 9,0*10-3 = 0,009
*INA Indicator Not Assessed
NEPD-3468-2072-EN giroflex 40
7 / 8
Additional Norwegian requirements
Greenhouse gas emissions from the use of electricity in the manufacturing phase
National production mix from import, low voltage (production of transmission lines, in addition to direct emissions and losses in grid) of applied electricity for the manufacturing
process (A3).
Electricity mix Data source Amount Unit
Energy, electricity, Poland: 1 kWh ecoinvent 3.6 1099,70 g CO2-ekv/kWh
Dangerous substances
The product contains no substances given by the REACH Candidate list or the Norwegian priority list.
Indoor environment
Greenguard Gold, Blue Angel
Additional environmental information
Key environmental indicators for variants for this EPD: Cradle to Gate analyse from A1 to A3
Global warming (kg Share of recycled
Variant number Total energy use (MJ)
CO2) material in product(%)
giroflex 40 with ALU starbase polished 80,16 1 108,48 32,17
giroflex 40 with ALU starbase black 80,64 1 117,15 32,12
giroflex 40 with plastic starbase 91,91 1 217,42 24,76
Key environmental indicators for options for this EPD: Cradle to Gate analyse from A1 to A3
Global warming (kg Share of recycled
Option number Total energy use (MJ)
CO2) material in product(%)
giroflex 40 - Armrests polished (set) 40,61 432,86 0,11
giroflex 40 - Armrests black (set) 42,11 448,93 0,11
giroflex 40 - headrest 3,36 50,17 6.31
giroflex 40 - packaging 7,21 83,19 59,40
Bibliography
ISO 14025:2010 Environmental labels and declarations - Type III environmental declarations - Principles and procedures.
ISO 14044:2006 Environmental management - Life cycle assessment - Requirements and guidelines.
EN 15804:2012+A1:2013 Environmental product declaration - Core rules for the product category of construction products.
ISO 21930:2017 Sustainability in buildings and civil engineering works - Core rules for environmental product declarations of construction products.
ecoinvent v3, Allocation, cut-off by classification, Swiss Centre of Life Cycle Inventories.
Iversen et al., (2018) eEPD v3.0 - Background information for EPD generator system. LCA.no report number 04.18
Vold et al., (2019) EPD generator for Norsk Industri, Background information for industry application and LCA data, LCA.no report number 06.19.
NPCR Part A: Construction products and services. Ver. 1.0. April 2017, EPD-Norge.
NPCR 026 Part B for Furniture. Ver. 2.0 October 2018, EPD-Norge.
Program operator and publisher Phone: +47 23 08 80 00
The Norwegian EPD Foundation e-mail: post@epd-norge.no
Post Box 5250 Majorstuen, 0303 Oslo,Norway web: www.epd-norge.no
Owner of the declaration Phone: 0047 98 25 68 30
Flokk AS e-mail: atle.messel@flokk.com
Drammensveien 145, 0277 Oslo web: https://www.flokk.com
Author of the Life Cycle Assessment Phone: +47 916 50 916
LCA.no AS e-mail: post@lca.no
Dokka 1C 1671 Kråkerøy web: www.lca.no
Developer of EPD generator Phone: +47 916 50 916
LCA.no AS e-mail: post@lca.no
Dokka 1C 1671 Kråkerøy web: www.lca.no
NEPD-3468-2072-EN giroflex 40
8 / 8
