Environmental product declaration
in accordance with ISO 14025 and EN 15804+A2
FIBOTHERM Trockenschüttung 1-5 round/crushed, Fibo ExClay Deutschland GmbH
Owner of the declaration: Program operator:
Leca International The Norwegian EPD Foundation
Product: Declaration number:
FIBOTHERM Trockenschüttung 1-5 round/crushed, Fibo
ExClay Deutschland GmbH Registration number:
Declared unit: Issue date:
1 m3
Valid to:
This declaration is based on Product Category Rules:
EPD Software:
CEN Standard EN 15804:2012+A2:2019 serves as core
The Norwegian EPD Foundation LCA.no EPD generator ID: 57877
PCR.
NPCR 012:2018 Part B for Thermal insulation products
1 / 11
General information
Product Owner of the declaration:
FIBOTHERM Trockenschüttung 1-5 round/crushed, Fibo ExClay Leca International
Deutschland GmbH Contact person: Tone Storbråten
Phone: +47 41 43 71 00
e-mail: info@leca.no
Program operator: Manufacturer:
Post Box 5250 Majorstuen, 0303 Oslo, Norway Leca International
The Norwegian EPD Foundation Årnesvegen 1
Phone: +47 23 08 80 00 2009 Nordby, Norway
web: post@epd-norge.no
Declaration number: Place of production:
Leca Denmark A/S
Randersvej 75 Hinge
8940 Randers Denmark, Denmark
This declaration is based on Product Category Rules: Management system:
CEN Standard EN 15804:2012+A2:2019 serves as core PCR. ISO 14001ISO 9001
NPCR 012:2018 Part B for Thermal insulation products
Statement of liability: Organisation no:
The owner of the declaration shall be liable for the underlying 918 799 141
information and evidence. EPD Norway shall not be liable with respect
to manufacturer information, life cycle assessment data and
evidences.​
Declared unit: Issue date:
1 m3 FIBOTHERM Trockenschüttung 1-5 round/crushed, Fibo ExClay
Deutschland GmbH
Declared unit with option: Valid to:
A1,A2,A3,A4,A5,C1,C2,C3,C4,D
Year of study:
2021
Functional unit: Comparability:
EPD of construction products may not be comparable if they not
comply with EN 15804:2012+A2:2019 and seen in a building context.
General information on verification of EPD from EPD tools: Development and verification of EPD:
Independent verification of data, other environmental information The declaration is created using EPD tool lca.tools ver EPD2022.03,
and the declaration according to ISO 14025:2010, § 8.1.3 and § 8.1.4. developed by LCA.no. The EPD tool is integrated in the company's
Verification of each EPD is made according to EPD-Norway’s management system, and has been approved by EPD Norway.
guidelines for verification and approval requiring that tools are i)
integrated into the company's environmental management system, ii) Developer of EPD: Ana Raquel Fernandes
the procedures for use of the EPD tool are approved by EPD-Norway,
Reviewer of company-specific input data and EPD:​ Tone Storbråten
and iii) the process is reviewed annually by an independent third
party verifier. See Appendix G of EPD-Norway's General Programme
Instructions for further information on EPD tools
Verification of EPD tool: Approved:
Independent third party verification of the EPD tool, background data
and test-EPD in accordance with EPDNorway's procedures and
guidelines for verification and approval of EPD tools.
Third party verifier:
Elisabet Amat - GREENIZE projects
(no signature required)
2 / 11
Product
Product description:
The EPD describes results for production of lightweight expanded clay aggregate, labelled FIBOTHERM, FIBOTHERM Trockenschüttung 1-5
round/crushed, from the factory in Lamstedt, Germany. Lightweight expanded clay aggregate is a granular ceramic material made from natural
clay. The clay mixed with organic material, dried and expanded to 3-4 times its original volume in rotary kilns at temperatures of about 1150 ° C.
The output lightweight expanded clay aggregate granules, in the range 0-32 mm, are sieved and blended into different grades of products and
distributed in bulk or in bags.
The main characteristic of expanded clay is low density combined with high strength. FIBOTHERM is a manufactured thermal insulation from
expanded clay lightweight aggregates. The density of FIBOTHERM Trockenschüttung 1-5 round/crushed is 450 kg/m³. The thermal conductivity is
0.12 W/mK. Further information or explanatory material may be obtained by contacting Fibo ExClay Deutschland GmbH.
Product specification
FIBOTHERM Trockenschüttung is a filling made of natural expanded clay with a grain size of 1-5 mm and is the sound- and thermal insulating
base for constructions that are under heavy load. It is characterized by high stability and low weight. FIBOTHERM Trockenschüttung is CE-certified
as a thermal insulation material according to EN 14063-1 and holds the Blauer Engel eco-label (low emission).
Materials Value Unit
Clay 92 %
Waste/bio raw materials 8 %
Lime < 0,5 %
Technical data:
Grading (Test method: EN 933-1): 1-5 mm
Loose bulk density (Test method: EN 1097-3): 450 Kg/m³
Reaction to fire (2000/605/EG): A1
Grain strength (Test method: EN 13055-1): 1,4 [N/mm2]
Compressive strength (Test method: EN 826): 60 [t/m2]
Thermal conductivity (Test method: EN 12667): 0,10 [W/(mK)]
Water suction height (Test method: EN 1097-10) > 270 [Hcap(mm)]
Market:
Germany
Reference service life, product
Not relevant.
Reference service life, building or construction works
Not relevant.
LCA: Calculation rules
Declared unit:
1 m3 FIBOTHERM Trockenschüttung 1-5 round/crushed, Fibo ExClay Deutschland GmbH
Cut-off criteria:
All major raw materials and all the essential energy is included. The production processes for raw materials and energy flows with very small
amounts (less than 1%) are not included. These cut-off criteria do not apply for hazardous materials and substances.
Allocation:
The allocation is made in accordance with the provisions of EN 15804+A2. Incoming energy and water and waste production in-house is allocated
equally among all products through mass allocation. Effects of primary production of recycled materials is allocated to the main product in which
the material was used. The recycling process and transportation of the material is allocated to this analysis.
Data quality:
Specific data for the product composition are provided by the manufacturer. The data represent the production of the declared product and were
collected for EPD development in the year of study. Background data is based on EPDs according to EN 15804 and different LCA databases. The
data quality of the raw materials in A1 is presented in the table below.
Materials Source Data quality Year
Lightweight Aggregate (LWA) Leca EPD 2022
3 / 11
System boundaries (X=included, MND=module not declared, MNR=module not relevant)
Construction Beyond the system
Product stage Use stage End of life stage
installation stage boundaries
A1 A2 A3 A4 A5 B1 B2 B3 B4 B5 B6 B7 C1 C2 C3 C4 D
X X X X X MND MND MND MND MND MND MND X X X X X
System boundary:
Additional technical information:
waR slairetam tropsnarT gnirutcafunaM tropsnarT ylbmessA e​sU ecnanetniaM riapeR tnemecalpeR tnemhsibrufeR lanoitarepO ygrene esu lanoitarepO esu retaw -eD noitcurtsnoc noitilomed tropsnarT etsaW gnissecorp lasopsiD -yrevoceR-esueR laitnetop-gnilcyceR
4 / 11
LCA: Scenarios and additional technical information
The following information describe the scenarios in the different modules of the EPD.
Capacity utilisation Value
Transport from production place to user (A4) Distance (km) Fuel/Energy Consumption Unit
(incl. return) % (Liter/tonne)
Truck, 16-32 tonnes, EURO 6 (km) 36,7 % 50 0,043 l/tkm 2,15
Assembly (A5) Unit Value
Blowing, Machine operation, diesel, > 18.64 kW
h/DU 0,03
(per hour)
Bulldozer, Machine operation, diesel, >=74.57 kW
h/DU 0,02
(per hour)
Crane, Machine operation, diesel, >=74.57 kW
h/DU 0,01
(per hour)
Vibrating plate (per liter diesel) L/DU 0,01
De-construction demolition (C1) Unit Value
Removal of LWA, Machine operation, diesel, >=
h/DU 0,04
74.57 kW (per hour)
Sorting per kg of LWA, for waste treatment after
kg/DU 450,00
removal (kg)
Capacity utilisation Value
Transport to waste processing (C2) Distance (km) Fuel/Energy Consumption Unit
(incl. return) % (Liter/tonne)
Truck, 16-32 tonnes, EURO 5 (km) 38,8 % 50 0,045 l/tkm 2,25
Waste processing (C3) Unit Value
Waste treatment, reuse of LWA (kg) kg 337,50
Disposal (C4) Unit Value
Disposal, landfilling of waste LWA (kg) kg 112,50
Benefits and loads beyond the system
Unit Value
boundaries (D)
Substitution of primary expanded clay (kg) kg 337,50
5 / 11
LCA: Results
The LCA results are presented below for the declared unit defined on page 2 of the EPD document.
Environmental impact
Indicator Unit A1 A2 A3 A4 A5 C1 C2 C3 C4 D
GWP-total
kg CO2 -
1,72E+02 7,43E-02 5,34E+00 3,68E+00 1,27E+00 8,67E-01 3,75E+00 0,00E+00 9,24E-01 -8,48E+01
eq
GWP-fossil
kg CO2 -
1,71E+02 7,42E-02 5,25E+00 3,68E+00 1,27E+00 8,67E-01 3,75E+00 0,00E+00 9,23E-01 -8,45E+01
eq
GWP-biogenic
kg CO2 -
9,54E-01 3,07E-05 8,41E-02 1,52E-03 2,39E-04 1,61E-04 0,00E+00 0,00E+00 1,08E-03 -2,08E-01
eq
GWP-luluc
kg CO2 -
1,34E-02 2,64E-05 5,33E-03 1,31E-03 9,96E-05 6,79E-05 1,31E-03 0,00E+00 2,27E-04 -3,30E-02
eq
kg
ODP CFC11 - 2,56E-06 1,68E-08 3,55E-07 8,33E-07 2,73E-07 1,86E-07 8,33E-07 0,00E+00 3,49E-07 -4,98E-06
eq
mol H+
AP 5,21E-01 2,13E-04 2,15E-02 1,06E-02 5,70E-03 3,16E-03 1,53E-02 0,00E+00 8,21E-03 -6,74E-01
-eq
EP-FreshWater kg P -eq 9,66E-03 5,93E-07 6,59E-04 2,94E-05 4,60E-06 3,13E-06 2,95E-05 0,00E+00 1,05E-05 -4,20E-03
EP-Marine kg N -eq 1,97E-01 4,22E-05 5,90E-03 2,09E-03 2,09E-03 1,05E-03 4,55E-03 0,00E+00 3,05E-03 -8,43E-02
mol N -
EP-Terrestial 2,20E+00 4,72E-04 7,39E-02 2,34E-02 2,31E-02 1,16E-02 5,02E-02 0,00E+00 3,37E-02 -1,02E+00
eq
kg
POCP NMVOC 5,25E-01 1,81E-04 1,77E-02 8,95E-03 6,70E-03 3,56E-03 1,54E-02 0,00E+00 9,63E-03 -2,74E-01
-eq
ADP- kg Sb -
1,33E-04 2,05E-06 3,75E-05 1,02E-04 1,94E-06 1,32E-06 1,01E-04 0,00E+00 8,31E-06 -1,12E-03
minerals&metals1 eq
ADP-fossil1 MJ 1,47E+03 1,12E+00 7,06E+01 5,56E+01 1,74E+01 1,18E+01 5,66E+01 0,00E+00 2,54E+01 -8,57E+02
WDP1 m3 7,21E+01 1,09E+00 5,96E+02 5,37E+01 3,70E+00 2,52E+00 5,39E+01 0,00E+00 1,57E+02 -1,59E+03
GWP-total = Global Warming Potential total; GWP-fossil = Global Warming Potential fossil fuels; GWP-biogenic = Global Warming Potential biogenic; GWP-luluc =
Global Warming Potential land use and land use change; ODP = Depletion potential of the stratospheric ozone layer; AP = Acidification potential, Accumulated
Exceedance; EP-freshwater = Eutrophication potential, fraction of nutrients reaching freshwater end compartment: EP-marine = Eutrophication potential, fraction of
nutrients reaching marine end compartment; EP-terrestrial = Eutrophication potential, Accumulated Exceedance; POCP = Formation potential of tropospheric ozone;
ADP-minerals&metals = Abiotic depletion potential for non-fossil resources; ADP-fossil = Abiotic depletion for fossil resources potential; WDP = Water (user)
deprivation potential, deprivation-weighted water consumption
"Reading example: 9,0 E-03 = 9,0*10-3 = 0,009"
*INA Indicator Not Assessed
1. The results of this environmental impact indicator shall be used with care as the uncertainties on these results are high or as there is limited experienced with the
indicator
Remarks to environmental impacts
Due to polluter-pay-principle, the emissions from waste are not included.
Biogenic carbon from biofuels are balanced to be zero since they have their input and output in the same module.
6 / 11
Additional environmental impact indicators
Indicator Unit A1 A2 A3 A4 A5 C1 C2 C3 C4 D
PM Disease incidence 9,66E-06 4,55E-09 2,84E-07 2,25E-07 9,99E-08 6,20E-08 2,48E-07 0,00E+00 1,75E-07 -6,28E-06
IRP2 kgBq U235 -eq 8,93E-01 4,91E-03 2,36E-01 2,43E-01 7,45E-02 5,08E-02 2,48E-01 0,00E+00 1,16E-01 -1,78E+00
ETP-fw1 CTUe 2,11E+03 8,32E-01 5,73E+01 4,12E+01 9,52E+00 6,48E+00 4,17E+01 0,00E+00 1,39E+01 -2,07E+03
HTP-c1 CTUh 1,72E-08 0,00E+00 1,58E-09 0,00E+00 1,08E-09 7,22E-10 0,00E+00 0,00E+00 5,63E-10 -3,78E-08
HTP-nc1 CTUh 1,64E-06 9,09E-10 5,66E-08 4,50E-08 8,04E-09 5,15E-09 4,50E-08 0,00E+00 1,00E-08 -1,02E-06
SQP1 dimensionless 2,48E+02 7,85E-01 1,56E+01 3,89E+01 2,21E+00 1,50E+00 3,90E+01 0,00E+00 9,78E+01 -1,19E+03
PM = Particulate Matter emissions; IRP = Ionizing radiation – human health; ETP-fw = Eco toxicity – freshwater; HTP-c = Human toxicity – cancer effects; HTP-nc =
Human toxicity – non cancer effects; SQP = Potential Soil Quality Index (dimensionless)
"Reading example: 9,0 E-03 = 9,0*10-3 = 0,009"
*INA Indicator Not Assessed
1. The results of this environmental impact indicator shall be used with care as the uncertainties on these results are high or as there is limited experienced with the
indicator
2. This impact category deals mainly with the eventual impact of low dose ionizing radiation on human health of the nuclear fuel cycle. It does not consider effects due
to possible nuclear accidents, occupational exposure nor due to radioactive waste disposal in underground facilities. Potential ionizing radiation from the soil, from
radon and from some construction materials is also not measured by this indicator.
7 / 11
Resource use
Indicator Unit A1 A2 A3 A4 A5 C1 C2 C3 C4 D
PERE MJ 1,42E+02 1,61E-02 1,08E+01 7,95E-01 9,41E-02 6,41E-02 7,99E-01 0,00E+00 9,09E-01 -2,32E+02
PERM MJ 0,00E+00 0,00E+00 0,00E+00 0,00E+00 0,00E+00 0,00E+00 0,00E+00 0,00E+00 0,00E+00 0,00E+00
PERT MJ 1,42E+02 1,61E-02 1,08E+01 7,95E-01 9,41E-02 6,41E-02 7,99E-01 0,00E+00 9,09E-01 -2,32E+02
PENRE MJ 1,47E+03 1,12E+00 7,06E+01 5,56E+01 1,74E+01 1,18E+01 5,70E+01 0,00E+00 2,54E+01 -8,57E+02
PENRM MJ 0,00E+00 0,00E+00 0,00E+00 0,00E+00 0,00E+00 0,00E+00 0,00E+00 0,00E+00 0,00E+00 0,00E+00
PENRT MJ 1,47E+03 1,12E+00 7,06E+01 5,56E+01 1,74E+01 1,18E+01 5,70E+01 0,00E+00 2,54E+01 -8,57E+02
SM kg 6,29E+01 0,00E+00 1,27E-03 0,00E+00 8,54E-03 5,82E-03 2,27E-02 0,00E+00 1,10E-02 -1,27E+00
RSF MJ 1,00E+01 5,75E-04 3,34E+00 2,85E-02 2,32E-03 1,58E-03 2,86E-02 0,00E+00 1,89E-02 -6,13E+00
NRSF MJ 3,31E+02 2,06E-03 3,66E-02 1,02E-01 3,41E-02 2,32E-02 1,02E-01 0,00E+00 4,07E-02 -4,80E+00
FW m3 1,43E-01 1,20E-04 3,20E-02 5,94E-03 8,95E-04 6,10E-04 5,96E-03 0,00E+00 3,12E-02 -5,70E-01
PERE = Use of renewable primary energy excluding renewable primary energy resources used as raw materials; PERM = Use of renewable primary energy resources used
as raw materials; PERT = Total use of renewable primary energy resources; PENRE = Use of non renewable primary energy excluding non-renewable primary energy
resources used as raw materials; PENRM = Use of non renewable primary energy resources used as raw materials; PENRT = Total use of non renewable primary energy
resources; SM = Use of secondary materials; RSF = Use of renewable secondary fuels; NRSF = Use of non-renewable secondary fuels; FW = Net use of fresh water
"Reading example: 9,0 E-03 = 9,0*10-3 = 0,009"
*INA Indicator Not Assessed
8 / 11
End of life - Waste
Indicator Unit A1 A2 A3 A4 A5 C1 C2 C3 C4 D
HWD kg 1,89E+00 5,79E-05 3,80E-02 2,87E-03 5,12E-04 3,49E-04 2,88E-03 0,00E+00 1,79E-03 -9,45E-02
NHWD kg 5,03E+00 5,46E-02 2,86E-01 2,70E+00 2,06E-02 1,40E-02 2,70E+00 0,00E+00 1,13E+02 -5,95E+00
RWD kg 9,48E-04 7,65E-06 3,19E-04 3,79E-04 1,21E-04 8,22E-05 3,85E-04 0,00E+00 1,65E-04 -2,55E-03
HWD = Hazardous waste disposed; NHWD = Non-hazardous waste disposed; RWD = Radioactive waste disposed
"Reading example: 9,0 E-03 = 9,0*10-3 = 0,009"
*INA Indicator Not Assessed
End of life - Output flow
Indicator Unit A1 A2 A3 A4 A5 C1 C2 C3 C4 D
CRU kg 0,00E+00 0,00E+00 0,00E+00 0,00E+00 0,00E+00 0,00E+00 0,00E+00 0,00E+00 0,00E+00 0,00E+00
MFR kg 2,54E-01 0,00E+00 2,12E-01 0,00E+00 8,26E-03 5,71E-03 3,17E-04 3,38E+02 1,00E-02 -1,03E+00
MER kg 4,32E-03 0,00E+00 2,82E-06 0,00E+00 1,55E-04 1,77E-05 1,89E-02 0,00E+00 1,89E-04 -6,16E-02
EEE MJ 4,88E+00 0,00E+00 6,75E-02 0,00E+00 8,92E-05 6,07E-05 2,19E-03 0,00E+00 1,56E-02 -1,34E-01
EET MJ 7,39E+01 0,00E+00 1,02E+00 0,00E+00 1,35E-03 9,19E-04 3,31E-02 0,00E+00 2,36E-01 -2,03E+00
CRU = Components for re-use; MFR = Materials for recycling; MER = Materials for energy recovery; EEE = Exported energy electrical; EET = Exported energy thermal
"Reading example: 9,0 E-03 = 9,0*10-3 = 0,009"
*INA Indicator Not Assessed
Biogenic Carbon Content
Indicator Unit At the factory gate
Biogenic carbon content in product kg C 0,00E+00
Biogenic carbon content in accompanying packaging kg C 0,00E+00
Note: 1 kg biogenic carbon is equivalent to 44/12 kg CO2
9 / 11
Additional requirements
Greenhouse gas emissions from the use of electricity in the manufacturing phase
National production mix from import, low voltage (production of transmission lines, in addition to direct emissions and losses in grid) of applied
electricity for the manufacturing process (A3).
Electricity mix Data source Amount Unit
Electricity, Germany (kWh) ecoinvent 3.6 585,93 g CO2-eq/kWh
Dangerous substances
The product contains no substances given by the REACH Candidate list or the Norwegian priority list.
Indoor environment
Additional Environmental Information
Additional environmental impact indicators required in NPCR Part A for construction products
Indicator Unit A1 A2 A3 A4 A5 C1 C2 C3 C4 D
GWPIOBC kg CO2 -eq 2,34E+01 7,43E-02 5,58E+00 3,68E+00 1,99E-01 1,98E-01 3,74E+00 0,00E+00 0,00E+00 -8,48E+01
GWP-IOBC: Global warming potential calculated according to the principle of instantaneous oxidation. In order to increase the transparency of biogenic carbon​
contribution to climate impact, the indicator GWP-IOBC is required as it declares climate impacts calculated according to the principle of instantaneous oxidation.​
GWP-IOBC is also referred to as GWP-GHG in context to Swedish public procurement legislation.
10 / 11
Bibliography
ISO 14025:2010 Environmental labels and declarations - Type III environmental declarations - Principles and procedures.
ISO 14044:2006 Environmental management - Life cycle assessment - Requirements and guidelines.
EN 15804:2012+A2:2019 Environmental product declaration - Core rules for the product category of construction products.
ISO 21930:2017 Sustainability in buildings and civil engineering works - Core rules for environmental product declarations of construction
products.
ecoinvent v3, Allocation, cut-off by classification, Swiss Centre of Life Cycle Inventories.
Iversen et al., (2021) eEPD v2021.09 Background information for EPD generator tool system verification, LCA.no Report number: 07.21
Vold et. al., (2022) EPD generator for NPCR 012 Thermal insulation, Background information for EPD generator application and LCA data, LCA.no
report number: 07.22.
NPCR Part A: Construction products and services. Ver. 2.0. April 2021, EPD-Norge.
NPCR 012 Part B for Part B for Thermal insulation products, Ver. 2.0, 31.03.2022, EPD Norway.
Program operator and publisher Phone: +47 23 08 80 00
The Norwegian EPD Foundation e-mail: post@epd-norge.no
Post Box 5250 Majorstuen, 0303 Oslo, Norway web: www.epd-norge.no
Owner of the declaration: Phone: +47 41 43 71 00
Leca International e-mail: info@leca.no
Årnesvegen 1, 2009 Nordby web: www.leca.no
Author of the Life Cycle Assessment Phone: +47 916 50 916
LCA.no AS e-mail: post@lca.no
Dokka 6B, 1671 web: www.lca.no
Developer of EPD generator Phone: +47 916 50 916
LCA.no AS e-mail: post@lca.no
Dokka 6B,1671 Kråkerøy web: www.lca.no
ECO Platform web: www.eco-platform.org
ECO Portal web: ECO Portal
11 / 11
