Environmental product declaration
in accordance with ISO 14025 and EN 15804+A2
PE Opto Cable Proctection Pipes in coil
Owner of the declaration: Program operator:
Pipelife Sverige AB The Norwegian EPD Foundation
Product: Declaration number:
PE Opto Cable Proctection Pipes in coil
Registration number:
Declared unit:
1 kg Issue date:
29.05.2023
This declaration is based on Product Category Rules:
CEN Standard EN 15804:2012+A2:2019 serves as core Valid to:
PCR 29.05.2028
The Norwegian EPD Foundation
NPCR Part A: Construction products and services
EPD Software:
LCA.no EPD generator ID: 63534
1 / 11
General information
Product Owner of the declaration:
PE Opto Cable Proctection Pipes in coil Pipelife Sverige AB
Contact person:
Phone: +46 513 22114
e-mail: yvette.lennartsson@pipelife.com
Program operator: Manufacturer:
Post Box 5250 Majorstuen, 0303 Oslo, Norway Pipelife Sverige AB
The Norwegian EPD Foundation
Phone: +47 23 08 80 00
web: post@epd-norge.no
Declaration number: Place of production:
Pipelife Sverige AB
Box 50
SE-524 02 Ljung , Sweden
This declaration is based on Product Category Rules: Management system:
CEN Standard EN 15804:2012+A2:2019 serves as core PCR EN ISO 9001:2015 and EN ISO 14001:2015
NPCR Part A: Construction products and services
Statement of liability: Organisation no:
The owner of the declaration shall be liable for the underlying SE556087042901
information and evidence. EPD Norway shall not be liable with respect
to manufacturer information, life cycle assessment data and
evidences.​
Declared unit: Issue date:
1 kg PE Opto Cable Proctection Pipes in coil 29.05.2023
Declared unit (cradle to gate) with option: Valid to:
A1-A3,A4,A5,C1,C2,C3,C4,D 29.05.2028
Year of study:
2022
Functional unit: Comparability:
EPD of construction products may not be comparable if they not
comply with EN 15804+A2 and seen in a construction context.
General information on verification of EPD from EPD tools: Development and verification of EPD:
Independent verification of data, other environmental information The declaration is created using EPD tool lca.tools ver EPD2022.03,
and the declaration according to ISO 14025:2010, § 8.1.3 and § 8.1.4. developed by LCA.no. The EPD tool is integrated in the company's
Verification of each EPD is made according to EPD-Norway’s management system, and has been approved by EPD Norway.
guidelines for verification and approval requiring that tools are i)
integrated into the company's environmental management system, ii) Developer of EPD: Yvette Lennartsson
the procedures for use of the EPD tool are approved by EPD-Norway,
Reviewer of company-specific input data and EPD: Bjørn Svensson
and iii) the process is reviewed annually by an independent third
party verifier. See Appendix G of EPD-Norway's General Programme
Instructions for further information on EPD tools
Verification of EPD tool: Approved:
Independent third party verification of the EPD tool, background data
and test-EPD in accordance with EPDNorway's procedures and
guidelines for verification and approval of EPD tools.
Third party verifier:
Michael M. Jenssen, Asplan Viak AS Håkon Hauan, CEO EPD-Norge
(no signature required)
2 / 11
Product
Product description:
Smooth PE cable protection pipes in short lenghts.
Low friction inner layer.
Products are UV stable.
Product specification
70005267, 70005275, 70005234, 70005260, 70005238, 70005242, 70005240, 70005268, 70005269, 70005271, 70005272, 70005273,
70005274
Product related data to be found at Pipelife Sverige AB product catalogue https://catalog.pipelife.com/se.
Materials kg %
Polyethylene (HDPE) 0,25 25,00
Plastic - Polyethylene (HDPE) 0,75 75,00
Total 1,00
Technical data:
PE material with density 960 kg/m3.
Market:
Europe, with scenario made for the Swedish market.
Reference service life, product
Lifetime on product calculated more than 100 years.
Reference service life, building
LCA: Calculation rules
Declared unit:
1 kg PE Opto Cable Proctection Pipes in coil
Cut-off criteria:
Allocation:
Data quality:
Specific data for the product composition are provided by the manufacturer. The data represent the production of the declared product and were
collected for EPD development in the year of study. Background data is based on EPDs according to EN 15804 and different LCA databases. The
data quality of the raw materials in A1 is presented in the table below.
Materials Source Data quality Year
Plastic - Polyethylene (HDPE) ecoinvent 3.6 Database 2019
Polyethylene (HDPE) ecoinvent 3.6 Database 2019
3 / 11
System boundaries (X=included, MND=module not declared, MNR=module not relevant)
Construction Beyond the system
Product stage Use stage End of life stage
installation stage boundaries
A1 A2 A3 A4 A5 B1 B2 B3 B4 B5 B6 B7 C1 C2 C3 C4 D
X X X X X MND MND MND MND MND MND MND X X X X X
System boundary:
Additional technical information:
waR slairetam tropsnarT gnirutcafunaM tropsnarT ylbmessA e​sU ecnanetniaM riapeR tnemecalpeR tnemhsibrufeR lanoitarepO ygrene esu lanoitarepO esu retaw -eD noitcurtsnoc noitilomed tropsnarT etsaW gnissecorp lasopsiD -yrevoceR-esueR laitnetop-gnilcyceR
4 / 11
LCA: Scenarios and additional technical information
The following information describe the scenarios in the different modules of the EPD.
A5 = 5 % product losses during installation are estimated by the company. According to NPCR 028, other activities such as excavating/backfilling
trenches and other additional materials are not included, these are expected to be included at construction level assessments.
C1 = According to NPCR 028, other activities such as excavating/backfilling trenches and other additional materials are not included, these are
expected to be included at construction level assessments. This module can therefore be included with zero impact.
C2 = Estimated transport of product 100 km.
C3 - C4 =Waste treatment of the product follows the default values provided in EN 50693, Product Category Rules for life cycle assessments of
electronic and electrical products and systems, table G.4. This table specified how different types of raw materials used in A1 will likely be treated
during the end-of-life of the product. Waste treatments in C3 include material recycling and incineration with and without energy recovery and fly
ash extraction. Disposal in C4 consist of landfilling of different waste fractions and of ashes.
D = The recyclability of metals and plastics allows the producers a credit for the net scrap that is produced at the end of a product’s life. The
benefits from recycling of net scrap are described in formula from EN 15804:2012+A2:2019. Substitution of heat and electricity generated by the
incineration with energy recovery of plastics is also calculated in module D.
Capacity utilisation Value
Transport from production place to user (A4) Distance (km) Fuel/Energy Consumption Unit
(incl. return) % (Liter/tonne)
Truck, over 32 tonnes, EURO 6 (km) 53,3 % 100 0,023 l/tkm 2,30
Assembly (A5) Unit Value
Product loss during installation (percentage of
Units/DU 0,05
cable pipe)
Capacity utilisation Value
Transport to waste processing (C2) Distance (km) Fuel/Energy Consumption Unit
(incl. return) % (Liter/tonne)
Truck, 16-32 tonnes, EURO 6 (km) 36,7 % 100 0,043 l/tkm 4,30
Waste processing (C3) Unit Value
Landfilling of ashes from incineration of
Polyethylene (PE), process per kg ashes and kg 0,38
residues (kg)
Waste treatment of polyethylene (PE),
incineration with energy recovery and fly ash kg 0,50
extraction (kg)
Disposal (C4) Unit Value
Landfilling of ashes from incineration of
Polyethylene (PE), process per kg ashes and kg 0,02
residues (kg)
Landfilling of plastic mixture (kg) kg 0,13
Benefits and loads beyond the system
Unit Value
boundaries (D)
Substitution of electricity (MJ) MJ 0,97
Substitution of thermal energy, district heating
MJ 14,67
(MJ)
5 / 11
LCA: Results
The LCA results are presented below for the declared unit defined on page 2 of the EPD document.
Environmental impact
Indicator Unit A1-A3 A4 A5 C1 C2 C3 C4 D
GWP-total kg CO2 -eq 1,23E+00 8,72E-03 1,31E-01 0 1,63E-02 1,53E+00 1,53E-02 -8,81E-02
GWP-fossil kg CO2 -eq 1,22E+00 8,71E-03 1,30E-01 0 1,63E-02 1,53E+00 1,53E-02 -8,50E-02
GWP-biogenic kg CO2 -eq 5,66E-03 3,73E-06 2,81E-04 0 6,76E-06 2,32E-05 1,79E-06 -1,76E-04
GWP-luluc kg CO2 -eq 3,13E-03 2,65E-06 1,54E-04 0 5,81E-06 4,93E-06 4,26E-07 -2,93E-03
ODP kg CFC11 -eq 1,07E-07 2,10E-09 3,72E-09 0 3,70E-09 3,32E-09 4,91E-10 -6,20E-03
AP mol H+ -eq 4,22E-03 2,80E-05 1,91E-04 0 4,69E-05 2,61E-04 1,31E-05 -7,01E-04
EP-FreshWater kg P -eq 2,65E-05 6,93E-08 1,29E-06 0 1,31E-07 3,99E-07 2,61E-08 -7,56E-06
EP-Marine kg N -eq 9,15E-04 6,14E-06 4,20E-05 0 9,29E-06 1,13E-04 1,94E-05 -2,29E-04
EP-Terrestial mol N -eq 1,02E-02 6,85E-05 4,59E-04 0 1,04E-04 1,24E-03 5,05E-05 -2,48E-03
POCP kg NMVOC -eq 3,64E-03 2,69E-05 1,64E-04 0 3,98E-05 3,05E-04 1,73E-05 -6,83E-04
ADP-minerals&metals1 kg Sb -eq 1,76E-05 1,55E-07 6,72E-07 0 4,51E-07 1,65E-07 1,47E-08 -8,46E-07
ADP-fossil1 MJ 3,11E+01 1,41E-01 1,45E+00 0 2,47E-01 2,83E-01 3,74E-02 -1,22E+00
WDP1 m3 9,31E+02 1,08E-01 4,66E+01 0 2,39E-01 2,21E+00 3,35E-01 -1,51E+01
GWP-total = Global Warming Potential total; GWP-fossil = Global Warming Potential fossil fuels; GWP-biogenic = Global Warming Potential biogenic; GWP-luluc =
Global Warming Potential land use and land use change; ODP = Depletion potential of the stratospheric ozone layer; AP = Acidification potential, Accumulated
Exceedance; EP-freshwater = Eutrophication potential, fraction of nutrients reaching freshwater end compartment: EP-marine = Eutrophication potential, fraction of
nutrients reaching marine end compartment; EP-terrestrial = Eutrophication potential, Accumulated Exceedance; POCP = Formation potential of tropospheric ozone;
ADP-minerals&metals = Abiotic depletion potential for non-fossil resources; ADP-fossil = Abiotic depletion for fossil resources potential; WDP = Water (user)
deprivation potential, deprivation-weighted water consumption
"Reading example: 9,0 E-03 = 9,0*10-3 = 0,009"
*INA Indicator Not Assessed
1. The results of this environmental impact indicator shall be used with care as the uncertainties on these results are high or as there is limited experienced with the
indicator
Remarks to environmental impacts
The products are produced on 100% renewable energy according mass balance principle.
6 / 11
Additional environmental impact indicators
Indicator Unit A1-A3 A4 A5 C1 C2 C3 C4 D
PM Disease incidence 4,78E-08 8,00E-10 1,91E-09 0 1,00E-09 1,62E-09 2,37E-10 -4,25E-08
IRP2 kgBq U235 -eq 2,53E-01 6,18E-04 1,22E-02 0 1,08E-03 1,05E-03 1,80E-04 -7,77E-03
ETP-fw1 CTUe 1,31E+01 1,03E-01 6,03E-01 0 1,83E-01 6,45E-01 5,09E-02 -6,61E+00
HTP-c1 CTUh 5,69E-10 0,00E+00 3,10E-11 0 0,00E+00 5,10E-11 2,00E-12 -1,22E-10
HTP-nc1 CTUh 1,40E-08 1,00E-10 7,04E-10 0 2,00E-10 1,92E-09 5,30E-11 -6,34E-09
SQP1 dimensionless 6,74E+00 1,62E-01 2,91E-01 0 1,73E-01 5,18E-01 1,33E-01 -8,13E+00
PM = Particulate Matter emissions; IRP = Ionizing radiation – human health; ETP-fw = Eco toxicity – freshwater; HTP-c = Human toxicity – cancer effects; HTP-nc =
Human toxicity – non cancer effects; SQP = Soil Quality (dimensionless)
"Reading example: 9,0 E-03 = 9,0*10-3 = 0,009"
*INA Indicator Not Assessed
1. The results of this environmental impact indicator shall be used with care as the uncertainties on these results are high or as there is limited experienced with the
indicator
2. This impact category deals mainly with the eventual impact of low dose ionizing radiation on human health of the nuclear fuel cycle. It does not consider effects due
to possible nuclear accidents, occupational exposure nor due to radioactive waste disposal in underground facilities. Potential ionizing radiation from the soil, from
radon and from some construction materials is also not measured by this indicator.
7 / 11
Resource use
Indicator Unit A1-A3 A4 A5 C1 C2 C3 C4 D
PERE MJ 4,73E+00 1,78E-03 2,36E-01 0 3,54E-03 1,40E-02 1,85E-03 -7,51E+00
PERM MJ 0,00E+00 0,00E+00 0,00E+00 0 0,00E+00 0,00E+00 0,00E+00 0,00E+00
PERT MJ 4,73E+00 1,78E-03 2,36E-01 0 3,54E-03 1,40E-02 1,85E-03 -7,51E+00
PENRE MJ -1,05E+01 1,41E-01 -6,27E-01 0 2,47E-01 2,83E-01 3,74E-02 -1,22E+00
PENRM MJ 4,25E+01 0,00E+00 2,12E+00 0 0,00E+00 0,00E+00 0,00E+00 0,00E+00
PENRT MJ 3,20E+01 1,41E-01 1,50E+00 0 2,47E-01 2,83E-01 3,74E-02 -1,22E+00
SM kg 7,51E-01 0,00E+00 3,76E-02 0 0,00E+00 0,00E+00 1,37E-05 0,00E+00
RSF MJ 7,49E-02 6,23E-05 3,70E-03 0 1,26E-04 3,58E-04 4,04E-05 -1,32E-03
NRSF MJ 4,74E-02 2,09E-04 4,15E-03 0 4,52E-04 3,82E-02 1,84E-03 -4,45E-01
FW m3 7,38E-02 1,61E-05 3,70E-03 0 2,64E-05 4,48E-04 4,37E-05 -9,05E-03
PERE = Use of renewable primary energy excluding renewable primary energy resources used as raw materials; PERM = Use of renewable primary energy resources used
as raw materials; PERT = Total use of renewable primary energy resources; PENRE = Use of non renewable primary energy excluding non-renewable primary energy
resources used as raw materials; PENRM = Use of non renewable primary energy resources used as raw materials; PENRT = Total use of non renewable primary energy
resources; SM = Use of secondary materials; RSF = Use of renewable secondary fuels; NRSF = Use of non-renewable secondary fuels; FW = Net use of fresh water
"Reading example: 9,0 E-03 = 9,0*10-3 = 0,009"
*INA Indicator Not Assessed
8 / 11
End of life - Waste
Indicator Unit A1-A3 A4 A5 C1 C2 C3 C4 D
HWD kg 1,67E-02 7,74E-06 1,74E-02 0 1,27E-05 3,17E-01 1,49E-02 -5,72E-05
NHWD kg 2,20E-01 1,23E-02 2,10E-02 0 1,20E-02 1,75E-01 1,33E-01 -2,87E-02
RWD kg 1,45E-04 9,66E-07 6,49E-06 0 1,68E-06 1,11E-06 2,42E-07 -6,37E-06
HWD = Hazardous waste disposed; NHWD = Non-hazardous waste disposed; RWD = Radioactive waste disposed
"Reading example: 9,0 E-03 = 9,0*10-3 = 0,009"
*INA Indicator Not Assessed
End of life - Output flow
Indicator Unit A1-A3 A4 A5 C1 C2 C3 C4 D
CRU kg 0,00E+00 0,00E+00 0,00E+00 0 0,00E+00 0,00E+00 0,00E+00 0,00E+00
MFR kg 1,76E-04 0,00E+00 9,35E-06 0 0,00E+00 0,00E+00 1,12E-05 0,00E+00
MER kg 1,09E-03 0,00E+00 2,51E-02 0 0,00E+00 5,00E-01 2,74E-07 0,00E+00
EEE MJ 7,37E-03 0,00E+00 4,88E-02 0 0,00E+00 9,70E-01 1,78E-05 0,00E+00
EET MJ 1,12E-01 0,00E+00 7,39E-01 0 0,00E+00 1,47E+01 2,69E-04 0,00E+00
CRU = Components for re-use; MFR = Materials for recycling; MER = Materials for energy recovery; EEE = Exported energy electrical; EET = Exported energy thermal
"Reading example: 9,0 E-03 = 9,0*10-3 = 0,009"
*INA Indicator Not Assessed
Biogenic Carbon Content
Indicator Unit At the factory gate
Biogenic carbon content in product kg C 0,00E+00
Biogenic carbon content in accompanying packaging kg C 0,00E+00
Note: 1 kg biogenic carbon is equivalent to 44/12 kg CO2
9 / 11
Additional requirements
Greenhouse gas emissions from the use of electricity in the manufacturing phase
National production mix from import, low voltage (production of transmission lines, in addition to direct emissions and losses in grid) of applied
electricity for the manufacturing process (A3).
Electricity mix Data source Amount Unit
Electricity, Sweden (kWh) ecoinvent 3.6 54,94 g CO2-eq/kWh
Dangerous substances
No substances given by the REACH Candidate list or the Norwegian priority list are intentionally added to the product.
Indoor environment
Additional Environmental Information
Additional environmental impact indicators required in NPCR Part A for construction products
Indicator Unit A1-A3 A4 A5 C1 C2 C3 C4 D
GWPIOBC kg CO2 -eq 1,18E+00 8,72E-03 1,28E-01 0 1,63E-02 1,53E+00 1,02E-03 -8,69E-02
GWP-IOBC: Global warming potential calculated according to the principle of instantaneous oxidation. In order to increase the transparency of biogenic carbon​
contribution to climate impact, the indicator GWP-IOBC is required as it declares climate impacts calculated according to the principle of instantaneous oxidation.​
GWP-IOBC is also referred to as GWP-GHG in context to Swedish public procurement legislation.
10 / 11
Bibliography
ISO 14025:2010 Environmental labels and declarations - Type III environmental declarations - Principles and procedures.
ISO 14044:2006 Environmental management - Life cycle assessment - Requirements and guidelines.
EN 15804:2012+A2:2019 Environmental product declaration - Core rules for the product category of construction products.
ISO 21930:2017 Sustainability in buildings and civil engineering works - Core rules for environmental product declarations of construction
products.
ecoinvent v3, Allocation, cut-off by classification, Swiss Centre of Life Cycle Inventories.
Iversen et al., (2021) eEPD v2021.09 Background information for EPD generator tool system verification, LCA.no rapportnummer: : 07.21.
Vold, et al., (2019) EPD generator for Pipelife - Background information for customer application and LCA data. report number 08.19
NPCR Part A: Construction products and services. Ver. 2.0. March 2021, EPD-Norge.
Program operator and publisher Phone: +47 23 08 80 00
The Norwegian EPD Foundation e-mail: post@epd-norge.no
Post Box 5250 Majorstuen, 0303 Oslo, Norway web: www.epd-norge.no
Owner of the declaration: Phone: +46 513 22114
Pipelife Sverige AB e-mail: yvette.lennartsson@pipelife.com
Box 50 , SE-524 02 Ljung web:
Author of the Life Cycle Assessment Phone: +47 916 50 916
LCA.no AS e-mail: post@lca.no
Dokka 6B, 1671 web: www.lca.no
Developer of EPD generator Phone: +47 916 50 916
LCA.no AS e-mail: post@lca.no
Dokka 6B,1671 Kråkerøy web: www.lca.no
ECO Platform web: www.eco-platform.org
ECO Portal web: ECO Portal
11 / 11
