Environmental Product
Declaration
In accordance with ISO 14025 and EN 15804 +A2
Owner of the declaration: AS+ Pipe LGY
Norsk Wavin AS
Program holder and publisher:
Wavin AS+ is a mineral-reinforced
The Norwegian EPD foundation
polypropylene (PP) low noise soil
and waste solution. The AS+ has a
Declaration number: unique material composition for
NEPD-3474-2069-EN
optimal noise reduction.
Registration Number:
NEPD-3474-2069-EN
Manufacturer
Wavin Germany Twist
Issue date: 27.05.2022
Valid to: 27.05.2027
The Norwegian EPD Foundation
Ver2-101122
General information
Product: Owner of the declaration:
AS+ Pipe LGY with socket; DN50, 70, 90, 100, 125, Norsk Wavin AS
150, 200, and light grey colour (LGY). Contact person: Matteo Tagliaferri
Phone: +31 623193684
Program Operator: e-mail: matteo.tagliaferri@wavin.com
The Norwegian EPD Foundation
Post Box 5250 Majorstuen, 0303 Oslo, Norway Manufacturer:
Tlf: +47 23 08 80 00 Wavin Germany Twist
e-mail: post@epd-norge.no Industriestraße 20, 49767, Twist, Germany
Phone: +49 5936 12 0
Declaration Number: e-mail: info@wavin.de
NEPD-3474-2069-EN
Place of production:
This declaration is based on Product Industriestraße 20, 49767, Twist, Germany
Category Rules:
Management system:
CEN standard EN 15804:2012+A2:2019 serves as
core PCR, supplied with NPCR Part A, Version 2.0. EN ISO 9001:2015 and EN ISO 14001:2015
Statements: Organisation no:
The owner of the declaration shall be liable for the 823355092
underlying information and evidence. EPD
Norway shall not be liable with respect to Issue date:
manufacturer, life cycle assessment data and 27.05.2022
evidences.
Valid to:
Declared unit:
27.05.2027
1 kg AS+ Pipe LGY
Year of study:
Declared unit with option:
2020
A1,A2,A3,A4,A5,C1,C2,C3,C4,D
Comparability:
Functional unit:
EPDs from other programmes than the Norwegian
Not applicable. EPD foundation may not be comparable.
Verification:
The EPD has been worked out by:
Independent verification of the declaration and
Lisa Overmars and Emma Thunnissen,
data, according to ISO14025:2010
Ecochain Technologies
internal external
Approved (Manager of EPD Norway)
Harry van Ewijk, SGS Search
Independent verifier approved by EPD Norway
EPD for the best environmental decision 2
Product
Product description:
Wavin AS+ is a mineral-reinforced polypropylene (PP) low noise soil and waste solution. The
AS+ has a unique material composition for improved noise performance. Optimal sound
reduction is guaranteed due to high density of material. Optimized three layer pipe structure for
low noise. The covered diameters are described in the Technical Data section.
Product specification:
A typical composition of the pipes, including packaging, covered by this EPD is as follows:
Materials %
PP 27%
Barium sulphate 51%
Filler 14%
Additives 8%
Rubber gasket & packaging 1%
The physical properties of the pipes covered in this EPD are:
• Density ~ 1,9 g/cm³
• E-Modul ~ 1800 N/mm²
• Linear coefficient of thermal expansion ~ 0,06 mm/mK
• Reaction to fire DIN 4102, B2 and EN13501 D-S3, d0
• Temperature Short-time load by 95°C and 90°C long-term stress
The color of the pipe is light grey (LGY): RAL7035
Technical data:
The declared unit of this EPD is 1 kg AS+ Pipe LGY. The results per kg are based on the product
‘AS+ Pipe LGY DN100 L=3 S/PL’ (‘base product’). The Table below provides the products
covered with this EPD. The selected base product is representative for all products described in
this Table; deviations of the LCA results of the other products compared to the base product are
not more than 10%. The list below provides the mass per 1 meter pipe (including packaging).
These masses should be used to calculate the LCA results per 1 meter pipe, by multiplying the
results presented on page 7-10 with the weight specified below.
Mass Mass
Product Product
(kg/meter) (kg/meter)
AS+ Pipe LGY DN50 L=0,15 S/PL 1.73 AS+ Pipe LGY DN100 L=0,5 S/PL 3.91
AS+ Pipe LGY DN50 L=0,25 S/PL 1.40 AS+ Pipe LGY DN100 L=1 S/PL 3.62
AS+ Pipe LGY DN50 L=0,5 S/PL 0.95 AS+ Pipe LGY DN100 L=2 S/PL 3.47
AS+ Pipe LGY DN50 L=1 S/PL 0.88 AS+ Pipe LGY DN100 L=2,7 S/PL 3.40
AS+ Pipe LGY DN50 L=2 S/PL 0.85 AS+ Pipe LGY DN100 L=3 S/PL 3.42
AS+ Pipe LGY DN50 L=2,7 S/PL 0.84 AS+ Pipe LGY DN125 L=0,25 S/PL 5.18
AS+ Pipe LGY DN50 L=3 S/PL 0.84 AS+ Pipe LGY DN125 L=0,5 S/PL 4.49
EPD for the best environmental decision 3
AS+ Pipe LGY DN70 L=0,15 S/PL 2.31 AS+ Pipe LGY DN125 L=1 S/PL 4.14
AS+ Pipe LGY DN70 L=0,25 S/PL 2.41 AS+ Pipe LGY DN125 L=2 S/PL 3.97
AS+ Pipe LGY DN70 L=0,5 S/PL 1.70 AS+ Pipe LGY DN125 L=2,7 S/PL 3.93
AS+ Pipe LGY DN70 L=1 S/PL 1.59 AS+ Pipe LGY DN125 L=3 S/PL 3.91
AS+ Pipe LGY DN70 L=2 S/PL 1.53 AS+ Pipe LGY DN150 L=0,5 S/PL 6.37
AS+ Pipe LGY DN70 L=2,7 S/PL 1.52 AS+ Pipe LGY DN150 L=1 S/PL 5.79
AS+ Pipe LGY DN70 L=3 S/PL 1.52 AS+ Pipe LGY DN150 L=2 S/PL 5.50
AS+ Pipe LGY DN90 L=0,15 S/PL 3.93 AS+ Pipe LGY DN150 L=2,7 S/PL 5.42
AS+ Pipe LGY DN90 L=0,25 S/PL 3.25 AS+ Pipe LGY DN150 L=3 S/PL 5.40
AS+ Pipe LGY DN90 L=0,5 S/PL 2.73 AS+ Pipe LGY DN200 L=0,25 S/PL 10.69
AS+ Pipe LGY DN90 L=1 S/PL 2.54 AS+ Pipe LGY DN200 L=0,5 S/PL 8.90
AS+ Pipe LGY DN90 L=2 S/PL 2.44 AS+ Pipe LGY DN200 L=1 S/PL 7.97
AS+ Pipe LGY DN90 L=2,7 S/PL 2.42 AS+ Pipe LGY DN200 L=2 S/PL 7.51
AS+ Pipe LGY DN90 L=3 S/PL 2.41 AS+ Pipe LGY DN200 L=2,7 S/PL 7.39
AS+ Pipe LGY DN100 L=0,25 S/PL 4.47 AS+ Pipe LGY DN200 L=3 S/PL 7.35
Market:
Europe, but the EPD is specific for Nordic countries.
Reference service life, product:
Lifetime on product calculated more than 100 year.
Reference service life, building:
LCA: Calculation rules
Declared unit:
1 kg AS+ Pipe LGY
Data quality:
For module A1, specific data for product compositions as provided by the manufacturer are
used. For module A2, transportation data of the raw materials used to the production site was
collected. For module A3, energy consumption and waste production data was collected for
production year 2020. The used background processes are derived from Ecoinvent 3.6.
Allocation:
Allocation was carried out in accordance with the provisions of the EN15804. All manufacturing
inputs (energy and auxiliary materials) at production site level are allocated to different
production processes, followed by allocation of the production processes to the products that
are produced using these processes through mass allocation. No secondary materials have been
used in the production process.
System boundary:
Modules A1-A5 and C1-D are included. The figure below shows a (simplified) process tree.
EPD for the best environmental decision 4
Cut-off criteria:
All relevant inputs and outputs - like emissions, energy and materials - have been taken into
account in this LCA. In accordance with EN15804, the total neglected input flows per module
does not exceed 5% of energy usage and mass.
LCA: Scenarios and additional technical information
The following information describe the scenarios in the different modules of the EPD.
Transport from production place to assembly/user (A4)
The transportation distance from Twist to Oslo was considered.
Capacity utilisation
Type Type of vehicle Distance KM Fuel/Energy consumption
(incl. return) %
Truck 50% Unspecified 945 0,027 l diesel/tkm
EPD for the best environmental decision 5
Boat 50% Ferry 163 0,0295 kg heavy fuel oil/tkm
Assembly (A5)
Product losses of 10% are considered. The installation is done manually, and therefore no
energy is needed.
Unit Value
Material loss kg 0,1
Packaging waste kg 0,003
End of Life (C1, C3, C4)
Demolition is done manually, and therefore no energy is needed. The considered waste
treatment for the pipe is 70% recycling, 20% incineration and 10% landfill.
Unit Value
Collected as mixed construction waste kg 1
Reuse kg 0
Recycling kg 0,70
Energy recovery kg 0,20
To landfill kg 0,10
Transport to waste processing (C2)
The considered distances are 50 km to landfill, 100 km for energy recovery, and 250 km for
recycling.
Capacity utilisation
Type Type of vehicle Distance KM Fuel/Energy consumption
(incl. return) %
Truck 50% Unspecified 199,8 0,027 l diesel/tkm
Benefits and loads beyond the system boundaries (D)
For the PP, barium sulphate and additives, 0,67 kg of saved virgin PP was considered per kg
material recycled (total of A5 en C3). For the filler, 0,67 kg of saved virgin filler was considered
per kg filler recycled. The benefits from exported energy were calculation from the energy
efficiencies for Northern countries reported by CEWEP, which is equal to an electrical
efficiencyof 11,0%, and a thermal efficiency of 72,6%. Energy recovery from all materials
(including rubber gasket and packaging) was considered. Substition of Norwegian electricity
mix and district heating mix was assumed.
Unit Value
Saving of virgin PP kg 0,44
Saving of virgin filler kg 0,07
Substition of electric energy MJ 0,28
Subsitition of thermal energy MJ 1,87
EPD for the best environmental decision 6
Additional technical information
Not applicable.
LCA: Results
The LCA results are presented below for the declared unit defined on page 2 of the EPD
document. Recalculation to results for pipes per meter can be done based on the technical data
specified on page 3 and 4.
System boundaries (X=included, MND= module not declared, MNR=module not
relevant)
Benefits
& loads
Assembly
Product stage Use stage End of life stage beyond
stage
system
boundary
n -
s la ir e wt a am R t r o p s n a r T g n ir u t c a fu n a M t r o p s n a r T y lb m e s s A e s U e c n a n e t n ia M r ia p e R t n e m e c a lp e R t n e m h s ib r u fe R la n o iy t ag rr eee pns Ou e la n o it ar re ete a ps w Ou n o io t cit ui rlo t sm ne od
c
-
t r o p s n a r T g n is s ee tc so ar Wp la s o p s iD g yn r eil v ec soy uc ce e RR --la it n e t o p
e e
D R
A1 A2 A3 A4 A5 B1 B2 B3 B4 B5 B6 B7 C1 C2 C3 C4 D
X X X X X X X X X X
Core environmental impact indicators
Indicator Unit A1-A3 A4 A5 C1 C2 C3 C4 D
GWP-total kg CO2 eq. 1,47E+00 1,41E-01 2,41E-01 0,00E+00 2,62E-02 6,85E-01 4,80E-03 -1,04E+00
GWP-fossil kg CO2 eq. 1,46E+00 1,41E-01 2,39E-01 0,00E+00 2,62E-02 6,82E-01 4,80E-03 -1,04E+00
GWP-biogenic kg CO2 eq. 6,49E-03 7,07E-05 1,06E-03 0,00E+00 1,59E-05 2,29E-03 9,19E-06 -4,04E-03
GWP-LULUC kg CO2 eq. 4,36E-03 5,45E-05 4,63E-04 0,00E+00 9,28E-06 2,04E-04 1,91E-07 -2,22E-04
ODP kg CFC11 eq. 1,08E-07 3,19E-08 1,91E-08 0,00E+00 6,04E-09 4,51E-08 2,96E-10 -3,46E-08
AP mol H⁺ eq. 6,21E-03 1,28E-03 8,77E-04 0,00E+00 1,49E-04 1,11E-03 6,92E-06 -3,18E-03
EP-freshwater kg P eq. 3,43E-05 1,08E-06 4,53E-06 0,00E+00 2,16E-07 9,68E-06 8,67E-09 -1,27E-05
EP-marine kg N eq. 1,21E-03 3,95E-04 1,96E-04 0,00E+00 5,34E-05 2,88E-04 3,98E-06 -5,47E-04
EP-terrestial mol N eq. 1,37E-02 4,37E-03 2,19E-03 0,00E+00 5,89E-04 3,18E-03 2,82E-05 -6,06E-03
kg NMVOC
POCP 4,81E-03 1,20E-03 7,19E-04 0,00E+00 1,68E-04 9,87E-04 9,01E-06 -2,83E-03
eq.
ADP-M&M kg Sb eq. 1,02E-04 3,30E-06 1,10E-05 0,00E+00 6,78E-07 3,98E-06 6,94E-09 -7,69E-06
ADP-fossil MJ 3,21E+01 2,11E+00 3,82E+00 0,00E+00 4,02E-01 3,53E+00 2,14E-02 -3,44E+01
WDP m³ 1,79E+00 6,09E-03 1,88E-01 0,00E+00 1,24E-03 7,89E-02 1,05E-04 -6,28E-01
EPD for the best environmental decision 7
GWP-total: Global Warming Potential; GWP-fossil: Global Warming Potential fossil fuels; GWP-biogenic:
Global Warming Potential biogenic; GWP-LULUC: Global Warming Potential land use and land use change;
ODP: Depletion potential of the stratospheric ozone layer; AP: Acidification potential, Accumulated
Exceedance; EP-freshwater: Eutrophication potential, fraction of nutrients reaching freshwater end
compartment; See “additional Norwegian requirements” for indicator given as PO4 eq. EP-marine:
Eutrophication potential, fraction of nutrients reaching freshwater end compartment; EP-terrestial:
Eutrophication potential, Accumulated Exceedance; POCP: Formation potential of tropospheric ozone; ADP-
M&M: Abiotic depletion potential for non-fossil resources (minerals and metals); ADP-fossil: Abiotic
depletion potential for fossil resources; WDP: Water deprivation potential, deprivation weighted water
counsumption
Additional environmental impact indicators
Indicator Unit A1-A3 A4 A5 C1 C2 C3 C4 D
Disease
PM 5,65E-08 1,16E-08 8,90E-09 0,00E+00 2,37E-09 1,82E-08 1,46E-10 -2,70E-08
incidence
IRP kBq U235 eq. 5,24E-02 9,22E-03 7,57E-03 0,00E+00 1,76E-03 1,22E-02 9,80E-05 -1,68E-02
ETP-fw CTUe 3,28E+02 1,68E+00 3,37E+01 0,00E+00 3,27E-01 7,76E+00 1,67E-02 -4,46E+00
HTP-c CTUh 5,56E-10 6,39E-11 1,09E-10 0,00E+00 1,16E-11 4,49E-10 4,91E-13 -1,86E-10
HTP-nc CTUh 1,59E-07 1,94E-09 1,68E-08 0,00E+00 3,90E-10 5,95E-09 1,01E-11 -5,35E-09
SQP Dimensionless 4,40E+00 1,65E+00 8,97E-01 0,00E+00 3,44E-01 2,51E+00 5,43E-02 -9,03E-01
PM: Particulate matter emissions; IRP: Ionising radiation, human health; ETP-fw: Ecotoxicity (freshwater);
ETP-c: Human toxicity, cancer effects; HTP-nc: Human toxicity, non-cancer effects; SQP: Land use related
impacts / soil quality
Classification of disclaimers to the declaration of core and additional environmental
impact indicators
ILCD
Indicator Disclaimer
classification
Global warming potential (GWP) None
ILCD type / level
Depletion potential of the stratospheric ozone layer (ODP) None
1
Potential incidence of disease due to PM emissions (PM) None
Acidification potential, Accumulated Exceedance (AP) None
Eutrophication potential, Fraction of nutrients reaching freshwater end
None
compartment (EP-freshwater)
Eutrophication potential, Fraction of nutrients reaching marine end
None
ILCD type / level compartment (EP-marine)
2
Eutrophication potential, Accumulated Exceedance (EP-terrestrial) None
Formation potential of tropospheric ozone (POCP) None
Potential Human exposure efficiency relative to U235 (IRP) 1
Abiotic depletion potential for non-fossil resources (ADP-minerals&metals) 2
Abiotic depletion potential for fossil resources (ADP-fossil) 2
ILCD type / level Water (user) deprivation potential, deprivation-weighted water consumption
2
3 (WDP)
Potential Comparative Toxic Unit for ecosystems (ETP-fw) 2
Potential Comparative Toxic Unit for humans (HTP-c) 2
EPD for the best environmental decision 8
Potential Comparative Toxic Unit for humans (HTP-nc) 2
Potential Soil quality index (SQP) 2
Disclaimer 1 – This impact category deals mainly with the eventual impact of low dose ionizing radiation on
human health of the nuclear fuel cycle. It does not consider effects due to
possible nuclear accidents, occupational exposure nor due to radioactive waste disposal in underground facilities.
Potential ionizing radiation from the soil, from radon and from some
construction materials is also not measured by this indicator.
Disclaimer 2 – The results of this environmental impact indicator shall be used with care as the uncertainties on
these results are high or as there is limited experienced with the indicator
Resource use
Parameter Unit A1-A3 A4 A5 C1 C2 C3 C4 D
RPEE MJ 2,91E+00 2,85E-02 3,24E-01 0,00E+00 5,77E-03 3,00E-01 7,58E-04 -4,54E-01
RPEM MJ 0,00E+00 0,00E+00 0,00E+00 0,00E+00 0,00E+00 0,00E+00 0,00E+00 0,00E+00
TPE MJ 2,91E+00 2,85E-02 3,24E-01 0,00E+00 5,77E-03 3,00E-01 7,58E-04 -4,54E-01
NRPE MJ 3,44E+01 2,24E+00 4,08E+00 0,00E+00 4,27E-01 3,76E+00 2,27E-02 -3,70E+01
NRPM MJ 0,00E+00 0,00E+00 0,00E+00 0,00E+00 0,00E+00 0,00E+00 0,00E+00 0,00E+00
TRPE MJ 3,44E+01 2,24E+00 4,08E+00 0,00E+00 4,27E-01 3,76E+00 2,27E-02 -3,70E+01
SM kg 0,00E+00 0,00E+00 0,00E+00 0,00E+00 0,00E+00 0,00E+00 0,00E+00 0,00E+00
RSF MJ 0,00E+00 0,00E+00 0,00E+00 0,00E+00 0,00E+00 0,00E+00 0,00E+00 0,00E+00
NRSF MJ 0,00E+00 0,00E+00 0,00E+00 0,00E+00 0,00E+00 0,00E+00 0,00E+00 0,00E+00
W m3 4,02E-02 2,24E-04 4,29E-03 0,00E+00 4,55E-05 2,36E-03 2,62E-05 -9,34E-03
RPEE Renewable primary energy resources used as energy carrier; RPEM Renewable primary energy
resources used as raw materials; TPE Total use of renewable primary energy resources; NRPE Non
renewable primary energy resources used as energy carrier; NRPM Non renewable primary energy
resources used as materials; TRPE Total use of non renewable primary energy resources; SM Use of
secondary materials; RSF Use of renewable secondary fuels; NRSF Use of non renewable secondary fuels; W
Use of net fresh water
End of life - Waste
Parameter Unit A1-A3 A4 A5 C1 C2 C3 C4 D
HW KG 1,51E-05 5,03E-06 2,87E-06 0,00E+00 1,03E-06 7,44E-06 2,56E-08 -6,10E-06
NHW KG 1,48E-01 1,17E-01 5,64E-02 0,00E+00 2,49E-02 1,69E-01 9,98E-02 -2,73E-02
RW KG 5,70E-05 1,44E-05 8,98E-06 0,00E+00 2,74E-06 1,53E-05 1,40E-07 -1,50E-05
HW Hazardous waste disposed; NHW Non hazardous waste disposed; RW Radioactive waste disposed
End of life – output flow
Parameter Unit A1-A3 A4 A5 C1 C2 C3 C4 D
CR kg 0,00E+00 0,00E+00 2,41E-06 0,00E+00 0,00E+00 0,00E+00 0,00E+00 0,00E+00
MR kg 0,00E+00 0,00E+00 6,99E-02 0,00E+00 0,00E+00 6,96E-01 0,00E+00 0,00E+00
MER kg 0,00E+00 0,00E+00 2,28E-02 0,00E+00 0,00E+00 2,01E-01 0,00E+00 0,00E+00
EEE MJ 0,00E+00 0,00E+00 0,00E+00 0,00E+00 0,00E+00 0,00E+00 0,00E+00 2,83E-01
EPD for the best environmental decision 9
ETE MJ 0,00E+00 0,00E+00 0,00E+00 0,00E+00 0,00E+00 0,00E+00 0,00E+00 1,87E+00
CR Components for reuse; MR Materials for recycling; MER Materials for energy recovery; EEE Exported
electric energy; ETE Exported thermal energy
Information describing the biogenic carbon content at the factory gate
Biogenic carbon content Unit Value
Biogenic carbon content in product kg C 0
Biogenic carbon content in the accompanying packaging kg C 0,0004
Additional Norwegian requirements
Greenhous gas emission from the use of electricity in the manufacturing phase
National production mix from import, low voltage (production of transmission lines, in addition
to direct emissions and losses in grid) of applied electricity for the manufacturing process(A3).
National electricity grid Unit Value
Hydroelectricity, average (Ecoinvent 3.6) kg CO2 -eq/kWh 0,0496
Additional environmental impact indicators required in NPCR Part A for construction
products
In order to increase the transparency of biogenic carbon contribution to climate impact, the
indicator for GWP has been sub-divided into the following:
GWP-IOBC Climate impacts calculated according to the principle of instantanious oxidation
GWP-BC Climate impacts from the net uptake and emission of biogenic carbon from each
module.
Indicator Unit A1-A3 A4 A5 C1 C2 C3 C4 D
GWP-IOBC kg CO2 eq. 1,46E+00 1,41E-01 2,40E-01 0,00E+00 2,62E-02 6,82E-01 4,79E-03 -1,04E+00
GWP-BC kg CO2 eq. 6,49E-03 7,07E-05 1,06E-03 0,00E+00 1,59E-05 2,29E-03 9,19E-06 -4,04E-03
GWP kg CO2 eq. 1,47E+00 1,41E-01 2,41E-01 0,00E+00 2,62E-02 6,85E-01 4,80E-03 -1,04E+00
GWP-IOBC Global warming potential calculated according to the principle of instantanious oxidation. GWP-
BC Global warming potential from net uptake and emissions of biogenic carbon from the materials in each
module. GWP Global warming potential
Hazardous substances
The declaration is based upon reference to threshold values and/or test results and/or material
safety data sheets provided to EPD verifiers. Documentation available upon request to EPD
owner.
✓ The product contains no substances given by the REACH Candidate list or the
Norwegian priority list.
□ The product contains substances given by the REACH Candidate list or the Norwegian
priority list that are less than 0,1 % by weight.
EPD for the best environmental decision 10
□ The product contain dangerous substances, more then 0,1% by weight, given by the
REACH Candidate List or the Norwegian Priority list, see table.
□ The product contains no substances given by the REACH Candidate list or the
Norwegian priority list. The product is classified as hazardous waste (Avfallsforskiften,
Annex III), see table.
Indoor environment
The product meets the requirements for low emissions.
Carbon footprint
Carbon footprint has not been worked out for the product.
EPD for the best environmental decision 11
Bibliography
ISO 14025:2010 Environmental labels and declarations - Type III environmental
declarations - Principles and procedures
ISO 14044:2006 Environmental management - Life cycle assessment -
Requirements and guidelines
EN 15804:2012+A2:2019 Sustainability of construction works - Environmental product
declaration - Core rules for the product category of construction
products
ISO 21930:2007 Sustainability in building construction – Environmental
declaration of building products
NPCR Part A Construction products and services. Ver. 2.0. March 2021, EPD-
Norge
CEWEP Results of Specific Data for Energy, R1 Plant Efficiency Factor and
NCV of 314 European Waste-to-Energy (WtE) Plants, CEWEP
Energy Report III (status 2007-2010), 2012, Reiman, D.O.
Program Operator tlf +47 23 08 80 00
The Norwegian EPD Foundation
Post Box 5250 Majorstuen, 0303 Oslo e-post: post@epd-norge.no
Norway web www.epd-norge.no
Publisher tlf +47 23 08 80 00
The Norwegian EPD Foundation
Post Box 5250 Majorstuen, 0303 Oslo e-post: post@epd-norge.no
Norway web www.epd-norge.no
Owner of the declaration tlf +4745190625
Norsk Wavin AS Fax
Karihaugveien 89, 1086, Oslo e-post: Invoice.no@wavin.com
Norway web www.wavin.com/nn-no
Author of the life cycle assessment tlf +31 (0)20 303 5777
Lisa Overmars Fax
H.J.E. Wenckebachweg 123, 1096 AM
e-post: lovermars@ecochain.com
Amsterdam
The Netherlands web www.ecochain.com
EPD for the best environmental decision 12
EPD for the best
environmental
decision
The Norwegian EPD foundation
www.epd-norge.no
